ver1 2015
ENVIRONMENTAL PRODUCT DECLARATION
in accordance with ISO 14025, ISO 21930 and EN 15804
Owner of the declaration: Flokk AS
Program operator: The Norwegian EPD Foundation
Publisher: The Norwegian EPD Foundation
Declaration number: NEPD-3715-2659-EN
Registration number: NEPD-3715-2659-EN
ECO Platform reference number: -
Issue date: 09.09.2022
Valid to: 09.09.2027
OFFECCT Thelma, Room divider
Flokk AS
www.epd-norge.no
NEPD-3715-2659-EN OFFECCT Thelma, Room divider (korr-090523)
1 / 8
General information
Product: Owner of the declaration:
OFFECCT Thelma, Room divider
Flokk AS
Contact person: Atle Thiis-Messel
Phone: 0047 98 25 68 30
e-mail: atle.messel@flokk.com
Program operator: Manufacturer:
Flokk AS
The Norwegian EPD Foundation
Drammensveien 145, 0277 Oslo
Pb. 5250 Majorstuen, 0303 Oslo
Norway
Phone: +47 23 08 80 00
e-mail: post@epd-norge.no
Declaration number: Place of production:
Flokk - Turek
NEPD-3715-2659-EN ul. Górnicza 8 62-700 Turek
Poland
ECO Platform reference number: Management system:
ISO 14001, ISO 9001, ISO 50001(Norway, Sweden)
This declaration is based on Product Category Rules: Organisation no:
No 928 902 749
CEN Standard EN 15804:2012+A1:2013 serves as core PCR
NPCR 026:2018 Part B for furniture
Statement of liability: Issue date: 09.09.2022
The owner of the declaration shall be liable for the underlying information and
evidence. EPD Norway shall not be liable with respect to manufacturer Valid to: 09.09.2027
information, life cycle assessment data and evidences.
Declared unit: Year of study:
1 Pcs OFFECCT Thelma, Room divider 2022
Declared unit with option: Comparability:
A1,A2,A3,A4 EPDs from programmes other than the Norwegian EPD Foundation may not be
comparable
Functional unit: Development and verification of EPD:
The declaration has been developed and verified using EPD tool lca.tools
ver EPD2020.11, developed by LCA.no AS. The EPD tool is integrated into
the company's environmental management system, and has been
approved by EPD-Norway
General information on verification of EPD from EPD tools:
Independent verification of data, other environmental information and Developer of EPD:
the declaration according to ISO 14025:2010, § 8.1.3 and § 8.1.4. Individual
third party verification of each EPD is not required when the EPD tool is i) Damian Bakowski
integrated into the company's environmental management system, ii) the
procedures for use of the EPD tool are approved by EPDNorway, and iii) Reviewer of company-specific input data and EPD:
the proccess is reviewed annualy. See Appendix G of EPD-Norway's
General Programme Instructions for further information on EPD tools. Arleta Derdziak
Verification of EPD tool: Approved:
Independent third party verification of the EPD tool, background data
Sign
and test-EPD in accordance with EPDNorway's procedures and guidelines
for verification and approval of EPD tools.
Erik Svanes, Norsus AS
(no signature required) Håkon Hauan, CEO EPD-Norge
Key environmental indicators Unit Cradle to gate A1 - A3
Global warming kg CO2 eqv 95,96
Total energy use MJ 1425,62
Amount of recycled materials % 49,36
NEPD-3715-2659-EN OFFECCT Thelma, Room divider (korr-090523)
2 / 8
Product
Market: Technical data:
Wordwide https://www.offecct.com/product/thelma-room-divider
Product description: Reference service life, product
The sound absorber Thelma is named after Pauline Deltour’s youngest
5 years
daughter, a name that is said to mean ‘divine protection’. “It has a
stylized simplicity with fabrics that are wrapped around it and create a Reference service life, building
tailored and elegant expression. At the same time, I’m struck by the
light-hearted playfulness that the sound absorber expresses; it feels
self-conscious and urban, but at the same time relaxed and unforced",
says Tobias Strålman , Design lead at Offecct.
Since our offices and ways of working have changed, towards
increased flexibility and more but smaller spaces for physical and digital
meetings. Thelma sound absorber are designed for use in such soft,
adaptable work spaces – and also come with smart accessories such as
a hook.
Product specification
Acoustic room divider upholstered in textile.
Frame, wheel and hook in lacquered metal. Black and white as
standard, Flexicolor as an option on request.
Recycled share in Recycled share in
Materials kg %
material (kg) material (%)
Metal - Aluminium 1,65 5,36 1,65 100,00
Metal - Steel 10,41 33,91 1,95 18,72
Textile - Polyester (PE) 3,49 11,36 2,84 81,54
Rubber, synthetic 0,12 0,38 0,00 0,00
Powder coating 0,28 0,91 0,00 0,00
Plastic - Nylon (PA) 0,02 0,06 0,00 0,00
Textile - Felt 4,81 15,67 3,74 77,70
Glue 0,18 0,59 0,01 2,83
Total: 20,95 10,18
LCA: Calculation rules
Declared unit: Allocation:
The allocation is made in accordance with the provisions of EN 15804. Effects
1 Pcs OFFECCT Thelma, Room divider
of primary production of recycled materials is allocated to the main product
Cut-off criteria: in which the material was used. The recycling process and transportation of
the material is allocated to this analysis.
All major raw materials and all the essential energy is included. The
production processes for raw materials and energy flows with very small
amounts (less than 1%) are not included. These cut-off criteria do not
apply for hazardous materials and substances.
Data quality:
Specific data for the product composition are provided by the manufacturer. They represent the production of the declared product and were collected for
EPD development in the year of study. Background data is based on registered EPDs according to EN 15804, Ostfold Research databases, ecoinvent and other
LCA databases. The data quality of the raw materials in A1 is presented in the table below.
Materials Source Data quality Year
Rubber, synthetic ecoinvent 3.4 Database 2015
Metal - Steel ecoinvent 3.3 Database 2016
Metal - Aluminium ecoinvent 3.4 Database 2017
Metal - Steel ecoinvent 3.4 Database 2017
Textile - Polyester (PE) ecoinvent 3.4 Database 2017
Powder coating ecoinvent 3.5 Database 2018
Plastic - Nylon (PA) ecoinvent 3.6 Database 2019
Process ecoinvent 3.6 Database 2019
Textile - Felt ecoinvent 3.6 Database 2019
Textile - Polyester (PE) ecoinvent 3.6 Database 2019
Database and
Glue Modified ecoinvent 3.6 2019
supplier
NEPD-3715-2659-EN OFFECCT Thelma, Room divider (korr-090523)
3 / 8
System boundary:
Additional technical information:
NEPD-3715-2659-EN OFFECCT Thelma, Room divider (korr-090523)
4 / 8
LCA: Scenarios and additional technical information
The following information describe the scenarios in the different modules of the EPD.
Transport from production place to user (A4)
Capacity utilisation Fuel/Energy
Type Type of vehicle Distance km Unit Value (l/t)
(incl. return) % consumption
Truck 38,8 % Truck, 16-32 tonnes, EURO 5 1000 0,044606 l/tkm 44,61
Railway l/tkm
Boat l/tkm
Other Transportation l/tkm
NEPD-3715-2659-EN OFFECCT Thelma, Room divider (korr-090523)
5 / 8
LCA: Results
The LCA results are presented below for the declared unit defined on page 2 of the EPD document.
System boundaries (X=included, MND=module not declared, MNR=module not relevant)
Construction Beyond the
Product stage installation User stage End of life stage . system
stage bondaries
A1 A2 A3 A4 A5 B1 B2 B3 B4 B5 B6 B7 C1 C2 C3 C4 . D
X X X X MND MND MND MND MND MND MND MND MND MND MND MND . MND
Environmental impact
Parameter Unit A1 A2 A3 A4
GWP kg CO 2 -eq 8,76E+01 2,27E+00 6,12E+00 3,36E+00
ODP kg CFC11 -eq 5,52E-06 4,27E-07 1,58E-07 6,20E-07
POCP kg C 2H 4-eq 2,79E-02 3,68E-04 1,39E-03 5,48E-04
AP kg SO 2 -eq 3,65E-01 8,66E-03 3,68E-02 1,07E-02
EP kg PO 3- -eq 6,43E-02 1,56E-03 4,47E-03 1,78E-03
4
ADPM kg Sb -eq 2,62E-03 4,60E-06 3,39E-07 1,02E-05
ADPE MJ 1,01E+03 3,47E+01 6,23E+01 5,06E+01
GWP Global warming potential; ODP Depletion potential of the stratospheric ozone layer; POCP Formation potential of tropospheric photochemical oxidants;
AP Acidification potential of land and water; EP Eutrophication potential; ADPM Abiotic depletion potential for non fossil resources; ADPE Abiotic depletion
potential for fossil resources
Reading example: 9,0 E-03 = 9,0*10-3 = 0,009
*INA Indicator Not Assessed
waR slairetam tropsnarT gnirutcafunaM tropsnarT ylbmessA esU ecnanetniaM riapeR tnemecalpeR tnemhsibrufeR lanoitarepO ygrene esu lanoitarepO esu
retaw
-eD noitcurtsnoc noitilomed tropsnarT etsaW gnissecorp lasopsiD -yrevoceR-esueR -gnilcyceR laitnetop
NEPD-3715-2659-EN OFFECCT Thelma, Room divider (korr-090523)
6 / 8
Resource use
Parameter Unit A1 A2 A3 A4
RPEE MJ 1,22E+02 6,42E-01 7,31E+00 7,38E-01
RPEM MJ 9,61E-01 0,00E+00 0,00E+00 0,00E+00
TPE MJ 1,23E+02 6,42E-01 7,31E+00 7,38E-01
NRPE MJ 1,19E+03 3,58E+01 6,58E+01 5,18E+01
NRPM MJ 5,77E+01 0,00E+00 0,00E+00 0,00E+00
TRPE MJ 1,25E+03 3,58E+01 6,58E+01 5,18E+01
SM kg 1,02E+01 0,00E+00 0,00E+00 0,00E+00
RSF MJ 2,87E-01 0,00E+00 0,00E+00 0,00E+00
NRSF MJ 3,04E-01 0,00E+00 0,00E+00 0,00E+00
W m3 9,39E-01 8,42E-03 3,28E-02 9,71E-03
RPEE Renewable primary energy resources used as energy carrier; RPEM Renewable primary energy resources used as raw materials; TPE Total use of renewable
primary energy resources; NRPE Non renewable primary energy resources used as energy carrier; NRPM Non renewable primary energy resources used as
materials; TRPE Total use of non renewable primary energy resources; SM Use of secondary materials; RSF Use of renewable secondary fuels; NRSF Use of non
renewable secondary fuels; W Use of net fresh water
Reading example: 9,0 E-03 = 9,0*10-3 = 0,009
*INA Indicator Not Assessed
End of life - Waste
Parameter Unit A1 A2 A3 A4
HW kg 1,32E-01 2,01E-05 3,14E-02 3,03E-05
NHW kg 5,93E+01 2,91E+00 2,28E+00 2,73E+00
RW kg INA* INA* INA* INA*
HW Hazardous waste disposed; NHW Non hazardous waste disposed; RW Radioactive waste disposed
Reading example: 9,0 E-03 = 9,0*10-3 = 0,009
*INA Indicator Not Assessed
End of life - Output flow
Parameter Unit A1 A2 A3 A4
CR kg 0,00E+00 0,00E+00 0,00E+00 0,00E+00
MR kg 2,92E-03 0,00E+00 7,67E-01 0,00E+00
MER kg 1,02E-01 0,00E+00 4,70E-03 0,00E+00
EEE MJ INA* INA* INA* INA*
ETE MJ INA* INA* INA* INA*
CR Components for reuse; MR Materials for recycling; MER Materials for energy recovery; EEE Exported electric energy; ETE Exported thermal energy
Reading example: 9,0 E-03 = 9,0*10-3 = 0,009
*INA Indicator Not Assessed
NEPD-3715-2659-EN OFFECCT Thelma, Room divider (korr-090523)
7 / 8
Additional Norwegian requirements
Greenhouse gas emissions from the use of electricity in the manufacturing phase
National production mix from import, low voltage (production of transmission lines, in addition to direct emissions and losses in grid) of applied electricity for the manufacturing
process (A3).
Electricity mix Data source Amount Unit
Energy, electricity, Poland: 1 kWh ecoinvent 3.6 1099,70 g CO2-ekv/kWh
Dangerous substances
The product contains no substances given by the REACH Candidate list or the Norwegian priority list.
Indoor environment
Additional environmental information
Key environmental indicators for options for this EPD: Cradle to Gate analyse from A1 to A3
Global warming (kg Share of recycled
Option number Total energy use (MJ)
CO2) material in product(%)
OFFECCT Thelma, Hook 0,55 7,71 19,58
OFFECCT Thelma, Packaging 11,07 142,96 96,99
Bibliography
ISO 14025:2010 Environmental labels and declarations - Type III environmental declarations - Principles and procedures.
ISO 14044:2006 Environmental management - Life cycle assessment - Requirements and guidelines.
EN 15804:2012+A1:2013 Environmental product declaration - Core rules for the product category of construction products.
ISO 21930:2017 Sustainability in buildings and civil engineering works - Core rules for environmental product declarations of construction products.
ecoinvent v3, Allocation, cut-off by classification, Swiss Centre of Life Cycle Inventories.
Iversen et al., (2018) eEPD v3.0 - Background information for EPD generator system. LCA.no report number 04.18
Vold et al., (2019) EPD generator for Norsk Industri, Background information for industry application and LCA data, LCA.no report number 06.19.
NPCR Part A: Construction products and services. Ver. 1.0. April 2017, EPD-Norge.
NPCR 026 Part B for Furniture. Ver. 2.0 October 2018, EPD-Norge.
Program operator and publisher Phone: +47 23 08 80 00
The Norwegian EPD Foundation e-mail: post@epd-norge.no
Post Box 5250 Majorstuen, 0303 Oslo,Norway web: www.epd-norge.no
Owner of the declaration Phone: 0047 98 25 68 30
Flokk AS e-mail: atle.messel@flokk.com
Drammensveien 145, 0277 Oslo web: https://www.flokk.com
Author of the Life Cycle Assessment Phone: +47 916 50 916
LCA.no AS e-mail: post@lca.no
Dokka 6B 1671 Kråkerøy web: www.lca.no
Developer of EPD generator Phone: +47 916 50 916
LCA.no AS e-mail: post@lca.no
Dokka 1C 1671 Kråkerøy web: www.lca.no
NEPD-3715-2659-EN OFFECCT Thelma, Room divider (korr-090523)
8 / 8
