1114 NEPD
Ver. 2 2015(17)
ENVIRONMENTAL PRODUCT DECLARATION
in accordance with ISO 14025, ISO 21930 and EN 15804
Owner of the declaration: Flügger Norway AS
Program operator: The Norwegian EPD Foundation
Publisher: The Norwegian EPD Foundation
Declaration number: NEPD-2322-1066-EN
Registration number: NEPD-2322-1066-EN
ECO Platform reference number: -
Issue date: 18.08.2020
Valid to: 18.08.2025
Flutex Pro 7
Flügger Norway AS
www.epd-norge.no
General information
Product: Owner of the declaration:
Flutex Pro 7™ Flügger Norway AS
contact person: Stine Rosendal Tangaa
phone: +45 40 64 75 98
e-mail: regulatoryaffairs@flugger.com
Program operator: Manufacturer:
The Norwegian EPD Foundation Flügger Denmark A/S
Pb. 5250 Majorstuen, 0303 Oslo
Tlf: +47 23 08 82 92
e-post: post@epd-norge.no
Declaration number: Place of production:
NEPD-2322-1066-EN Vejlevej 150
6000 Kolding, Denmark
ECO Platform reference number: Management system:
ISO 14001:2015 (DK011198)
ISO 9001:2015 (DK0012451)
This declaration is based on PCR: Org. no.:
NS-EN 15804:2012+A1:2013 serves as core PCR. 45240118
Product descriptions based on "IBU PCR Part B for coatings
with organic binders". This also applies to products with
inorganic binders.
Issue date:
Statement of liability: 18.08.2020
The owner of the declaration shall be liable for the underlying
informationandevidence.EPDNorwayshallnotbeliablewith
respect to manufacturer information, life cycle assessment
data and evidences. Valid to:
18.08.2025
Declared unit: Year of study:
2020
Declared unit with option: Comparability:
EPD of construction products may not be comparable if they
1 kg Flutex Pro 7 paint delivered to main warehouse in Norway
do not comply with NS-EN 15804+A1:2013 and seen in a
building context.
Functional unit: Author of the Life Cycle Assessment:
Gaylord Booto og Lars G. F. Tellnes
NORSUS AS
Verification:
Independent verification of data, other environmental
information and the declaration according to ISO14025:2010, §
8.1.3 and § 8.1.4
internal external
Approved
Third party verifier:
Erik Svanes, Senior Researcher
(Independent verifier approved by EPD Norway)
NEPD-2322-1066_Flutex-Pro-7_ENG verif 2/9
Product
Product description: Technical data:
Flutex Pro 7 is a water based, 100% acrylic wall paint for Density: 1,4 kg/l:
indoor use. The paint gives a matt surface with visible gloss, Solids by volume: 44,1%
uniform finish and an even structure. EU VOC limit value for product (Cat. A/a): 30 g/l
Product VOC max. 10 g/l
Flutex Pro 7 is ecolabelled with the Nordic Swan and EU
Ecolabel. Nominal spreading rate: 8 m2/l
Wet film thickness: 125 µm
Flutex Pro 7 is recommended for premises with high functional Dry film thickness: 55 µm
requirements, where the surface is exposed to dirt and wear
and tear. Withstands cleaning, including spot cleaning with soft The most representative and worst case formulation is chosen
brush, water and cloth. forthisEPD.Forproductswithaselectionofcolours,thiswill
be the formulation with the highest content of titanium dioxide.
For information on Green Building Standard credits and
Ecolabels, see "Additional Information" on page 4. The product packaging is based on an average sized plastic
packaging.
For safety, health and environmental conditions, see the
Product specification:
Safety Data Sheet for the declared product on
Life cycle assessment carried out for the white variant, which is
www.flugger.no.
estimated to have the greatest environmental impact.
For information on technical data, application and use of the
The material composition of the declared product:
product,seetheTechnicalDataSheetandFDV(Forvaltning,
Materials %
Drift og Vedlikehold) for the declared product on
Water 15-25
www.flugger.no
Binder 35-45
Extender 15-25
Titanium dioxide 10-20 Market:
Solvent < 0,1 Scandinavia and Europe
Additive < 2
Biocide < 0,1 Reference service life, product
The reference service life of the product is highly dependent
Packaging kg on the conditions of use.
Wooden packaging - pallet 0.000667
Plastic packaging - pallet 0.00021 Estimated service life, object
Plastic packaging 0.03335 The coated object is not declared.
LCA: Calculation rules
Declared unit: System boundary:
Flutex Pro 7™ The flow chart below illustrates the system boundaries for the
analysisaccordingtothemoduleprincipleinNS-EN15804.The
analysis is carried out from cradle-to-gate (A1-A3), including
module A4 transport to market.
A1 A2 A3 A4 A5 B1-B7 C1-C4 D
Raw materials Transport Production Transport to Application and Usephase Endof life Benefits of
market installation recovery
Preassemblyof
raw materials
Rawmaterial Transport of
extraction and raw materials
production Dispersionof
pigments
Transportof Module not Module not Module not Module not
product to declared declared declared declared
market
Mixing
Packaging Transport of
production packaging
QCcheck and
adjustment
Fillingand
labelling
Systemboundaries«Cradle-to-gate»
System boundary for this EPD
NEPD-2322-1066_Flutex-Pro-7_ENG verif 3/9
System boundary for this EPD
Data quality:
The CEPE database is used as basis for the rawmaterial composition. Specific datafor theproduct compositionand rawmaterial
amountshasbeenprovidedbythemanufacturerandrepresentstheproductionofthedeclaredproduct.Datafortheproductionsite
werecollectedin2020considering2019asthereferenceyear. RemainingdataisbasedonEcoinventv3.5,butadjustedtoimprove
representativeness. All energy consumption in the database is assumed not to be used as raw material.
Cut-off criteria: Allocation:
Allmajorrawmaterialsandessentialenergyisincluded.Someraw Theallocationismadeinaccordancewiththeprovisionsof
materialshavebeenmodelledusingequivalent substances(proxy NS-EN15804+A1:2013.Incomingenergy,waterandwaste
data). This does not apply for hazardous materials and productionin-houseisprimarilyallocatedequallyamongall
substances. Thus, 100% of the total product content is included. products through mass allocation. The recycling process
and transportation of the material is allocated to this
analysis.
Additional information:
The declared product contributes to Green Building Standard credits by meeting the following specific requirements:
-Emission criteria according to EN 15251 and EN 16000 9:2006 (<0,2 mg/m2/h after 28 days)
-Nordic Swan Ecolabel (3096 0024)
-EU Ecolabel (SE/044/002)
-Properties criteria in BASTA (2020:A1)
BREEAM®NOR (2016)
Hea 02: VOC content for Interior matt walls and ceilings (30 g/l) (EU Directive 2004/42/CE) and emission criteria (ISO 16000-series).
Mat01:TheproductcontainsnosubstancesontheNorwegianTechnicalCheckList(A20),whichexceedsthelimitvalueforhealthand
environment.
Additional certificates and approvals may be available on request.
NEPD-2322-1066_Flutex-Pro-7_ENG verif 4/9
LCA: Scenarios and additional technical information
The following information describe the scenarios in the different modules of the EPD.
The only declared module after the factory gate is A4 transport to market.
Transport is carried out in two steps, from production in Kolding to warehouse in Bollebygd and from Bollebygd to Oslo.
Transport from production place to user (A4)
Capacity utilisation (incl. Fuel/Energy
Type Type of vehicle Distance km Unit
return) % consumption
Truck 53.00 % >32t, EURO 6 537 0.0192 kg/tkm
Truck 53.00 % >32t, EURO 6 338 0.0192 kg/tkm
Boat
Other
Construction/Installation (A5) Use (B1)
Unit Value Unit Value
Auxiliary kg Relevant emissions during use kg
Water consumption m3
Electricity consumption kWh
Other energy carriers MJ
Material loss kg
Dust in the air kg
VOC emissions kg
Maintenance (B2)/Repair (B3) Replacement (B4)/Refurbishment (B5)
Unit Value Unit Value
Maintenance cycle* Replacement cycle*
Auxiliary kg Electricity consumption kWh
Other resources kg Replacement of worn parts
Water consumption m3 * Value or refence shelf-life
Electricity consumption kWh
Other energy carriers MJ
Material loss kg
VOC emissions kg
Operational energy (B6) and water consumption (B7) End of life (C1, C3, C4)
Unit Value Unit Value
Water consumption m3 Hazardous waste disposed kg
Electricity consumption kWh Collected as mixed construction waste kg
Other energy carriers MJ Reuse kg
Power output of equipment kW Recycling kg
Energy recovery kg
Til landfill kg
Transport to waste processing (C2)
Capacity utilisation (incl. Fuel/Energy
Type Type of vehicle Distance km Unit Value (l/t)
return) % consumption
Truck
Railway
Boat
Other
NEPD-2322-1066_Flutex-Pro-7_ENG verif 5/9
LCA: Results
System boundaries (X=included, MND=module not declared, MNR=module not relevant)
Beyond the
Construction/
Product stage User stage End of life stage system
installation stage
boundaries
s la ire ta m w a R tro p s n a rT g n iru tc a fu n a M tro p s n a rT /n o itc u rts n o Ce g a ts n o ita lla ts n i e s U e c n a n e tn ia M ria p e R tn e m e c a lp e R tn e m h s ib ru fe R e s u y g re n e la n o ita re p O e s u re ta w la n o ita re p O
n
o itilo m e d /n o itc u rts n o c e tro p s n a rT g n is s e c o rp e ts a W la s o p s id e ts a W
-g
n ilc y c e r/y re v o c e r/e s u ela itn e to p
D R
A1 A2 A3 A4 A5 B1 B2 B3 B4 B5 B6 B7 C1 C2 C3 C4 D
X X X X MND MND MND MND MND MND MND MND MND MND MND MND MND
Environmental impact
Parameter Unit A1 A2 A3 A4
GWP kg CO 2 -eq. 1,87E+00 3,84E-02 1,28E-01 7,53E-02
ODP kg CFC11-eq. 2,17E-07 7,16E-09 8,17E-09 1,51E-08
POCP kg C 2H 4 -eq. 1,07E-03 6,29E-06 5,07E-05 1,18E-05
AP kg SO 2 -eq. 1,25E-02 1,25E-04 1,04E-03 1,99E-04
EP kg PO 43--eq. 1,52E-03 2,06E-05 2,60E-04 2,73E-05
ADPM kg Sb -eq. 9,73E-06 1,06E-07 7,88E-06 1,47E-07
ADPE MJ 3,05E+01 5,88E-01 1,24E+00 1,24E+00
GWP Global warming potential; ODP Depletion potential of the stratospheric ozone layer; POCP Formation potential of tropospheric
photochemical oxidants; AP Acidification potential of land and water; EP Eutrophication potential; ADPM Abiotic depletion potential for non fossil
resources; ADPE Abiotic depletion potential for fossil resources
NEPD-2322-1066_Flutex-Pro-7_ENG verif 6/9
Resource use
Parameter Unit A1 A2 A3 A4
RPEE MJ 1,50E+00 6,54E-03 5,64E-01 1,33E-02
RPEM MJ 0,00E+00 0,00E+00 2,64E-02 0,00E+00
TPE MJ 1,50E+00 6,54E-03 5,91E-01 1,33E-02
NRPE MJ 3,00E+01 5,98E-01 1,60E+00 1,26E+00
NRPM MJ 3,70E+00 0,00E+00 0,00E+00 0,00E+00
TRPE MJ 3,37E+01 5,98E-01 1,60E+00 1,26E+00
SM kg 0,00E+00 0,00E+00 0,00E+00 0,00E+00
RSF MJ 0,00E+00 0,00E+00 0,00E+00 0,00E+00
NRSF MJ 0,00E+00 0,00E+00 0,00E+00 0,00E+00
W m3 2,64E-01 1,14E-04 1,23E-03 2,71E-04
RPEERenewableprimaryenergyresourcesusedasenergycarrier;RPEMRenewableprimaryenergyresourcesusedasrawmaterials;TPE
Total use of renewable primary energy resources; NRPE Non renewable primary energy resources used as energy carrier; NRPM Non
renewable primary energy resources used as materials; TRPE Total use of non renewable primary energyresources; SM Use of secondary
materials; RSF Use of renewable secondary fuels; NRSF Use of non renewable secondary fuels; W Use of net fresh water
End of life - Waste
Parameter Unit A1 A2 A3 A4
HW kg 3,69E-05 3,77E-07 3,79E-04 7,28E-07
NHW kg 6,14E-01 4,10E-02 1,68E-01 1,13E-01
RW kg 1,59E-04 4,04E-06 6,75E-06 8,55E-06
HW Hazardous waste disposed; NHW Non hazardous waste disposed; RW Radioactive waste disposed
End of life - Output flow
Parameter Unit A1 A2 A3 A4
CR kg 0,00E+00 0,00E+00 0,00E+00 0,00E+00
MR kg 0,00E+00 0,00E+00 2,06E-03 0,00E+00
MER kg 0,00E+00 0,00E+00 3,57E-05 0,00E+00
EEE MJ 0,00E+00 0,00E+00 2,53E-03 0,00E+00
ETE MJ 0,00E+00 0,00E+00 2,71E-02 0,00E+00
CR Components for reuse; MR Materials for recycling; MER Materials for energy recovery; EEE Exported electric energy; ETE Exported thermal
energy
Reading example: 9,0 E-03 = 9,0*10-3 = 0,009
NEPD-2322-1066_Flutex-Pro-7_ENG verif 7/9
Additional requirements
Greenhouse gas emissions from the use of electricity in the manufacturing phase
Nationalproductionmixfromimport,lowvoltage(productionoftransmissionlines,inadditiontodirectemissionsandlossesingrid)
of applied electricity for the manufacturing process (A3). Background data ispresented inthe table below. Characterisationfactors
from NS-EN 15804:2012+A1:2013 is used.
Electricity mix Data source Value Unit
Electricity, Denmark (kWh) ecoinvent 3.5 367 g CO -eq./kWh
2
Dangerous substances
The product contains no substances given by the REACH Candidate list or the Norwegian priority list
The product contains substances given by the REACH Candidate list <0,1 weight%
The product contains substances given by the REACH Candidate list or the Norwegian priority list, see table above
The product contains no substances given by the REACH Candidate list or the Norwegian priority list. The product is
characterised as hazardous waste (acc. to the Waste Directive, Appendix III), se table above.
Indoor environment
The declared product is emission tested according to the ISO-16000 series (2006).
NEPD-2322-1066_Flutex-Pro-7_ENG verif 8/9
Bibliography
BASTA (2020) Properties criteria - BASTA - in accordance with Regulation (EC) No 1272/2008 (CLP), ed. A1
Booto and Tellnes (2020): LCA-report for Flugger AS. Report OR.25.20 from NORSUS, Kråkerøy, Norway.
BREEAM®NOR (2016) BREEAM-NOR for new constructions 2016, SD 5075NOR, version 1.1. The Norwegian Green
Building Council
CEPE v3.0 Raw materials LCI database for the European coatings and printing ink industries
Dahlgren,L., Jelse,K., Skenhall,S.A., Ljungkvist,H., Westerdahl,J., Stripple,H., Högberg,J. and Rydberg,T. (2014). Raw materials LCI
database for the European coatings and printing ink industries-Documentation of datasets v.2.0, IVLU4859, August 2014
Dahlgren,L., Stripple,H., Oliveira,F., Rydberg,T., and Zhang,Y. (2016). Raw materials LCI database for the European coatings and
printing ink industries - Documentation of data sets v. 3.0, IVL U5659, May 2016.
Ecoinvent v3.5 Alloc Rec, Swiss Centre of Life Cycle Inventories. www.ecoinvent.ch
EN 15251 (2007) Indoor environmental input parameters for design and assessment of energy performance of
buildings addressing indoor air quality, thermal environment, lighting and acoustics. CEN, Brussels
EU Directive 2004/42/CE The limitation of emissions of volatile organic compounds due to the use of organic solvents in
certain paints and varnishes and vehicle refinishing products
EU Ecolabel SE/044/002
IBU PCR Part B Requirements on the EPD for Coatings with organic binders. v1.7, January 2019
ISO 16000-series Indoor air standards for VOCs sampling and determination, i.e. 9 (2006)
NS-EN ISO 14025:2010 Environmental labels and declarations - Type III environmental declarations - Principles and
procedures
NS-EN ISO 14044:2006 Environmental management - Life cycle assessment - Requirements and guidelines
NS-EN 15804:2012+A1:2013 Environmental product declaration - Core rules for the product category of construction products
NS-EN PCR Part A Construction Products and Services. Version 1.0. EPD Norge
REACH Candidate List (2018) Candidate List of substances of very high concern for Authorisation IAW Article 59(10) of the REACH
Regulation
Nordic Ecolabel 3096 0024
Technical Check List (A20) and Miljøgiftlisten, The Norwegian Environment Agency
Norwegian Priority List (2018)
Program operator and publisher phone: +47 977 22 020
The Norwegian EPD Foundation
Post Box 5250 Majorstuen, 0303 Oslo e-mail: post@epd-norge.no
Norway web www.epd-norge.no
Owner of the declaration phone: +47 23 30 21 90
Flügger Norway AS
Waldemar Thranes gate 84B e-mail: regulatoryaffairs@flugger.com
0175 Oslo, Norway web www.flugger.com
Author of the Life Cycle Assessment phone: +47 69 35 11 00
Gaylord Booto og Lars G. F. Tellnes fax: +47 69 34 24 94
NORSUS AS e-mail: post@norsus.no
Stadion 4, 1671 Kråkerøy, Norge web www.norsus.no
NEPD-2322-1066_Flutex-Pro-7_ENG verif 9/9
