Environmental Product
Declaration
In accordance with ISO 14025 and EN 15804 +A1
NTech inward opening windows 105/80 – ND, NS, NB (with
aluminium cladding)
Owner of the declaration:
NorDan AS Product name:
Program holder and publisher: NTech inward opening
windows 105/80 – ND, NS,
NB (with aluminium
The Norwegian EPD foundation
Declaration number: cladding)
NEPD-3451-2058-EN Manufacturer:
Registration Number:
NorDan AS
NEPD-3451-2058-EN
Issue date:
Valid to:
02.05.2022
The Norwegian 02.05.2027
EPD Foundation
General information
Product: Owner of the declaration:
NTech inward opening windows 105/80 – ND, NS, NB (with NorDan AS
aluminium cladding) Kontaktperson: Fredrik Jonsson
Tlf: +46 (0) 10-130 01 78
e-post: fredrik.jonsson@nordan.se
Program holder: Manufacturer:
The Norwegian EPD Foundation NorDan AS Moi,
Post Box 5250 Majorstuen, 0303 Oslo Moi, Rogaland, Norway
Tlf: +47 977 22 020
e-mail: post@epd-norge.no Phone: +47 51 40 40 00
Declaration number: Place of production:
NEPD-3451-2058-EN Moi, Rogaland, Norway
ECO Platform registration number: Management system:
NS-ISO 9001:2015, NS-EN ISO 14001:2015
This declaration is based on Product Category Rules:
CEN Standard EN 15804 serves as core PCR NPCR014:2019
version 3.0 Part B for Windows and doors Org. no.:
NO 979 776 233 MVA
Declaration of responsibility: Issue date:
The owner of the declaration shall be responsible for the 02.05.2022
underlying information and evidence. EPD Norway shall not
be responsible with regard to manufacturer information, life
cycle data and evidence.
Valid to:
02.05.2027
Declared unit: Year of study:
2021
Declared unit with option: Comparability:
EPD of construction products may not be comparable if they
are not comply with NS-EN 15804 and seen in a building
context.
Functional unit: The EPD has been worked out by:
1 window measuring 1.23 m x 1.48 m (reference window based Roja Modaresi
on EN 14351-1) with an expected service life of 60 years, with Norsk Treteknisk Institutt
aluminium cladding. with an essential parameter U-value =
0,81(W/m2K).Conversion factor is 66.77 [Kg/FU].
Verification:
Independent verification of the declaration and data,
according to ISO14025:2010
internal external
Approved
Third party verifier:
signiture
Gaylord K. Booto PhD., Senior Research Scientist, NORSUS AS
(Independent verifier approved by EPD Norway)
NEPD-3451-2058-EN NTech inward opening windows 105/80 – ND, NS, NB (with aluminium cladding)
2/9
Product
Product description: Technical data:
Windows with inward opening sash, tilt and turn, side and bottom Inward opening window. Triple glazed, 105mm frame with 8mm
hinged for use in exterior walls of domestic and commercial aluminium cladding, 80mm sash. Manufactured in accordance
buildings. The scope is NorDan 105 mm windows with sash and with ISO9001:2015 and NS-EN ISO 14001:2015. The product
timber frame with aluminium cladding. complies with the requirements of the Norwegian Door and
Window control. Uwin 0,81W/m2K. Certified: BBA, Secured by
Design, SP Sitac “P”.
Product specification:
25% of aluminium and 18% of glass is produced from recycled The total weight of the product is 66.77 kg. 2.4 kg of material is
material. used for aluminium cladding. The packaging has an average
Product group ND, NS, NB is covered in this EPD. The highest weight of 3.2 kg.
amount for constituent material has been used.
Materialer kg %
Pine timber 16.58 24.83
Glass 41.76 62.55
Spacer 0.74 1.11
Triple glazed Butyl 0.02 0.03 Market:
unit Sealant 1.09 1.63 Europe, but scenarios beyond cradle to gate are based
Argon gas 0.07 0.10 on the situation in the Norwegian market.
Absorbent 0.02 0.03
Paint 0.57 0.85
Aluminium 1.80 2.70
Plastic 0.16 0.24
Gasket 0.43 0.64
Metal- Steel alloys 1.07 1.60 Reference service life:
Sealant and Glue 0.08 0.12 The reference service life is 60 years for aluminium cladding
Aluminium 2.31 3.47 timber frame.
Additional for
Plastic 0.03 0.05
alu clad
Metals 0.03 0.05
Total weight of the product 66.77 100
Wood packaging 3.1
Steel packaging 0.05
Plastic packaging 0.08
Paper, cardboard packaging
Total weight with packaging 70.00
LCA: Calculation rules
Functional unit: System boundary:
1 window measuring 1.23 m x 1.48 m (reference window based on All modules are included. Below is a technical flowchart for
EN 14351-1) with an expected service life of 60 years, with the production line at NorDan. Modul D is calculated with
aluminium cladding. with an essential parameter U-value = energy substitution and explained in the scenarios.
0,81(W/m2K).Conversion factor is 66.77 [Kg/FU].
NEPD-3451-2058-EN NTech inward opening windows 105/80 – ND, NS, NB (with aluminium cladding)
3/9
Data quality Cut-off criteria:
Data is representative of year 2019 and was collected in 2020-2021. All raw materails and energy use is included. Where data was
Data is taken from processes from Ecoinvent 3.1-3.7. Some available for infrastructure from Ecoinvent, it is included.
processes are based on Ecoinvent v3.1 (2014) and v3.2 (2015), but Example: ‘Metal working factory'. In the production process,
all upstream processes are v3.4 (2017)-3.5 (2018). Remaining data raw materials and energy of low amounts are not included
is based on Ecoinvent v3.7 (2020). "Allocation cut-off by (<1%). These cut-off rules do not apply to dangerous
classification" adjusted to improve representativeness. substances.
Allocation: Calculations of biogenic carbon:
Allocation is done in accordance with the provisions of EN 15804. Sequestration and release of biogenic carbon is included
Allocation of energy, water and waste from production is calculated according to EN 16485:2014. This is based on the modularity
by a physical allocation factor based on the manufacturer input. For principle in EN 15804:2012 that specifies that the emissions
waste produced at the manufacturing, the burdens for reuse, shall be accounted in the module that they occur. The amount
recycling and recovery is allocated by using this allocation factor. of carbon dioxide sequestrated is calulated in accordance to
EN 16449:2014. Timber comes from sustainable forestry and
has FSC certified traceability.
LCA: Scenarios and additional technical information
The following information describe the scenarios in the different modules of the EPD
An average distance of 300 km with truck is used within Norway. The transportation from production to construction site is based on a
scenario where the product is transported on a large lorry to a radius of 250 km to a warehouse. Transport from warehouse to a
construction site is assumed to be 50 km on a medium truck.
Transport from production place to assembly/user (A4)
Type Capacity utilisation Type of vehicle Distance km Fuel/Energy Fuel/Energy
(incl. return) % consumption pr tkm consumption pr km
Truck 53 EURO5, >32 tonn 250 0.023 l/tkm 0.31 l/km
Truck 26 EURO5, 16-32 tonn 50 0.045 l/tkm 0.25 l/km
Installation (A5)
Unit Value According to the report from EPD-Norge ‘Harmonising the
Auxiliary kg 0 documentation of scenarios beyond cradle to gate, EN 15804’ there is
Water consumption m3 0 no loss on site during construction activities. The window products in
Electricity consumption MJ 0 this EPD are painted and surface treated in the production and not at
Other energy carriers MJ 0 the building site. Therefore, there is only 2 items left in this module. 1)
Material loss kg 0 Waste treatment of packaging which is considered in the EPD
Output materials from waste treatment kg 3.23 calculations. 1) Energy use during installation. This can be varied
Dust in the air kg 0 depending on the floor, type of building and several other unknown
parameters, and therefore ignored in the calculation.
Maintenance (B2)/Repair (B3)
The maintenance scenario included cleaning, painting and change of
Unit IGU. Cleaning is performed three times per year. It is calculated with
Value
1,5 dl of detergent and 3 litres of water each year. Windows with
Detergents kg 9
aluminium cladding are assumed to be painted 3 times during its
Water consumption l 180
lifetime from inside. It is assumed that 5 gr of lubricating oil is used
Lubricating oil kg 0.30
every year for fittings and moving parts. The glazing unit is changed
Paint kg 0.55 once during the lifetime for the windows with aluminium cladding. No
Transport tkm 2.95 repair is assumed during the product lifetime.
Glazing unit kg 43.70
Synthetic rubber kg 0.43
Transport (IGU) tkm 12.53
NEPD-3451-2058-EN NTech inward opening windows 105/80 – ND, NS, NB (with aluminium cladding)
4/9
Replacement (B4)/Refurbishment (B5)
*Number or RSL (Reference Service Life). The window has RSL of 60
Unit Value years for with aluminium cladding. Therefore, for windows with 60
Replacement cycle* yr 60 years RSL, it is assumed to replace the insulated glass unit after 30
Electricity consumption kWh 0 years (See Module B4). There is no need for refurbishment during the
Replacement of worn parts 0 0 product lifetime.
(C1) As there are no data for de-construction, it is assumed no activites in C1 in this study. The windows are assumed to be treated as
mixed waste and sent to incineration. The combustible materials are then energy recovered, while glass is assumed to end up in the
bottom ash and then landfilled. The metals are usually sorted out of the bottom ash and then recycled, but there is no data of the share
which are recycled and therefore standard values from Ecoinvent is utilized.
The transport of window as waste is calculated based on a scenario with 50 km distance.
Transport to waste processing (C2)
Type Capacity utilisation Type of vehicle Distance km Fuel/Energy Fuel/Energy
(incl. return) % consumption pr tkm consumption pr km
Truck 44 Unspecified 50 0.03l/tkm 0.28 l/km
Windows are assumed to be sorted as mixed construction waste and treated with incineration with energy recovery. However, The
manufacturer has documented the recycling potentials for its product in the Construction Product Declaration eBVD.
NorDan ND Dreh-kipp Säkerhetsfönster Trä/Alu 105, ID: C-SE556294452901-80 URL:
https://www.ebvd.org/BMI/Document/Export/4305/0/Pdf
In the documentation, Chapter 10, the specific material recovery, and energy recovery potential is reported for the product.
End of Life (C1, C3, C4)
Unit Value
Hazardous waste disposed kg 0
Collected as mixed construction waste kg 66.77
Reuse kg 0
Recycling kg 2.02
Energy recovery kg 64.74
To landfill kg 0.00
The benefits beyond life cycle has been modelled based on the output flows from module C3. This includes energy from incineration and
scrap metal recovered from the ashes. The amount recovered metal is assumed to avoid production of primary metals in accordance to
6.4.3.3 in EN 15804. The exported energy is substituting Norwegian district heating mix and electricity mix. Inventory processes causing
substitution of avoided virgin raw materials has be constructed for each material.
Benefits and loads beyond the system boundaries (D)
Unit Value
Substitution of electricity MJ 26.7
Substitution of thermal energy MJ 252.3
Substitution of raw materials kg 2.2
NEPD-3451-2058-EN NTech inward opening windows 105/80 – ND, NS, NB (with aluminium cladding)
5/9
LCA: Results
Global warming potential in A1-A3 includes sequestration of CO2 as carbon in the wood. The same amount is accounted as an
emission in module C3. Additionally, it is included sequestration in the wood packaging. This is accounted as an emission in module
A5. The flow of biogenic carbon for the system is presented in page 9.
System boundaries (X = included)
Beyond the
Construction and
Product stage Use stage End of Life stage system
installation stage
boundaries
X X X X X X X
Environmental impact With alu clad
B1 B4
GWP kg CO -ekv 1.01E+02 2.24E+00 0.00E+00 0.00E+00 0.00E+00
2
ODP kg CFC11-ekv 7.54E-06 4.30E-07 1.00E+00 0.00E+00 0.00E+00
POCP 0.00E+00 2.00E+00 0.00E+00 0.00E+00
AP kg SO -ekv 6.16E-01 5.77E-03 0.00E+00 3.00E+00 0.00E+00 0.00E+00
2
EP kg PO 3--ekv 7.92E-02 8.04E-04 0.00E+00 4.00E+00 0.00E+00 0.00E+00
4
ADPM 0.00E+00 5.00E+00 0.00E+00 0.00E+00
ADPE 0.00E+00 6.00E+00 0.00E+00 0.00E+00
D
GWP -3.51E+01
ODP kg CFC11-ekv 0.00E+00 0.00E+00 0.00E+00 8.69E-08 -1.08E-06
POCP kg C H -ekv 0.00E+00 0.00E+00 5.99E-05 2.63E-04 1.23E-04 -1.25E-02
2 4
kg SO -ekv 0.00E+00 -1.95E-01
2
EP kg PO 3--ekv 2.48E-04 5.52E-04 -1.82E-02
4
1.28E+01
slairetam
waR
tropsnarT
gnirutcafunaM
tropsnarT
noitallatsni
noitcurtsnoC
egats esU
ecnanetniaM
riapeR
tnemecalpeR tnemhsibrufeR
esu
ygrene
lanoitarepO
esu
retaw
lanoitarepO
noitcurtsnoc-eD
noitilomed tropsnarT
gnissecorp
etsaW
lasopsiD
-yrevoceR-esueR laitnetop
gnilcyceR
A1 A2 A3 A4 A5 B1 B2 B3 B4 B5 B6 B7 C1 C2 C3 C4 D
X X X X X X X X X X
Parameter Unit A1-A3 A4 A5 B2 B3 B5
4.55E+00 0.00E+00 6.60E+01
0.00E+00 0.00E+00 1.97E-06
kg C H -ekv 2.21E-01 2.72E-04 0.00E+00 1.64E-02
2 4
0.00E+00 2.28E-01
0.00E+00 3.33E-02
kg Sb-ekv 2.74E-03 6.14E-06 0.00E+00 6.09E-04
MJ 1.55E+03 3.53E+01 0.00E+00 9.39E+02
Parameter Unit B6 B7 C1 C2 C3 C4
kg CO -ekv 0.00E+00 0.00E+00 0.00E+00 4.74E-01 3.41E+01 5.34E-01
2
4.29E-08 1.41E-07
0.00E+00
AP 0.00E+00 0.00E+00 1.50E-03 4.02E-03 2.98E-03
0.00E+00 0.00E+00 0.00E+00 1.25E-03
ADPM kg Sb-ekv 0.00E+00 0.00E+00 0.00E+00 1.60E-06 1.06E-06 1.07E-06 -5.00E-05
ADPE MJ 0.00E+00 0.00E+00 0.00E+00 7.17E+00 7.95E+01 -3.30E+02
GWP Global warming potential; ODP Depletion potential of the stratospheric ozone layer; POCP Formation potential of tropospheric
photochemical oxidants; AP Acidification potential of land and water; EP Eutrophication potential; ADPM Abiotic depletion potential for non fossil
resources; ADPE Abiotic depletion potential for fossil resources.
NEPD-3451-2058-EN NTech inward opening windows 105/80 – ND, NS, NB (with aluminium cladding)
6/9
Resource use with alu clad
Parameter Unit A1-A3 A4 A5 B1 B2 B3 B4 B5
RPEE MJ 7.7E+02 4.4E-01 0.0E+00 0.0E+00 7.1E+01 0.0E+00 0.0E+00 0.0E+00
RPEM MJ 3.3E+02 0.0E+00 0.0E+00 0.0E+00 0.0E+00 0.0E+00 0.0E+00 0.0E+00
TPE MJ 1.1E+03 4.4E-01 0.0E+00 0.0E+00 7.1E+01 0.0E+00 0.0E+00 0.0E+00
NRPE MJ 1.7E+03 3.6E+01 0.0E+00 0.0E+00 1.0E+03 0.0E+00 0.0E+00 0.0E+00
NRPM MJ 9.1E+01 0.0E+00 0.0E+00 0.0E+00 7.3E+01 0.0E+00 0.0E+00 0.0E+00
TRPE MJ 1.8E+03 3.6E+01 0.0E+00 0.0E+00 1.1E+03 0.0E+00 0.0E+00 0.0E+00
SM kg 1.2E+00 0.0E+00 0.0E+00 0.0E+00 0.0E+00 0.0E+00 0.0E+00 0.0E+00
RSF MJ 2.0E-01 0.0E+00 0.0E+00 0.0E+00 8.9E-03 0.0E+00 0.0E+00 0.0E+00
NRSF MJ 2.1E-01 0.0E+00 0.0E+00 0.0E+00 8.6E-02 0.0E+00 0.0E+00 0.0E+00
W m3 3.4E+00 4.1E-03 0.0E+00 0.0E+00 7.9E-01 0.0E+00 0.0E+00 0.0E+00
Resource use with alu clad
Parameter Unit B6 B7 C1 C2 C3 C4 D
RPEE MJ 0.0E+00 0.0E+00 0.0E+00 9.8E-02 2.8E+02 1.9E-01 -1.6E+02
RPEM MJ 0.0E+00 0.0E+00 0.0E+00 0.0E+00 -2.8E+02 0.0E+00 0.0E+00
TPE MJ 0.0E+00 0.0E+00 0.0E+00 9.8E-02 6.4E-01 1.9E-01 -1.6E+02
NRPE MJ 0.0E+00 0.0E+00 0.0E+00 7.3E+00 8.0E+01 1.3E+01 -3.4E+02
NRPM MJ 0.0E+00 0.0E+00 0.0E+00 0.0E+00 -7.5E+01 0.0E+00 0.0E+00
TRPE MJ 0.0E+00 0.0E+00 0.0E+00 7.3E+00 4.5E+00 1.3E+01 -3.4E+02
SM kg 0.0E+00 0.0E+00 0.0E+00 0.0E+00 0.0E+00 0.0E+00 0.0E+00
RSF MJ 0.0E+00 0.0E+00 0.0E+00 0.0E+00 4.3E-01 0.0E+00 -1.0E+02
NRSF MJ 0.0E+00 0.0E+00 0.0E+00 0.0E+00 2.8E-01 0.0E+00 -6.7E+01
W m3 0.0E+00 0.0E+00 0.0E+00 7.9E-04 1.3E-02 1.2E-02 -5.8E-01
RPEE Renewable primary energy resources used as energy carrier; RPEM Renewable primary energy resources used as raw materials; TPE
Total use of renewable primary energy resources; NRPE Non renewable primary energy resources used as energy carrier; NRPM Non renewable
primary energy resources used as materials; TRPE Total use of non renewable primary energy resources; SM Use of secondary materials; RSF
Use of renewable secondary fuels; NRSF Use of non renewable secondary fuels; W Use of net fresh water.
End of life-Waste with alu clad
Parameter Unit A1-A3 A4 A5 B1 B2 B3 B4 B5
HW kg 3.32E+00 1.93E-03 0.00E+00 0.00E+00 1.90E+00 0.00E+00 0.00E+00 0.00E+00
NHW kg 3.69E+01 2.77E+00 0.00E+00 0.00E+00 9.56E+00 0.00E+00 0.00E+00 0.00E+00
RW kg 2.23E-02 2.47E-04 0.00E+00 0.00E+00 1.84E-02 0.00E+00 0.00E+00 0.00E+00
End of life-Waste with alu clad
Parameter Unit B6 B7 C1 C2 C3 C4 D
HW kg 0.00E+00 0.00E+00 0.00E+00 3.82E-04 5.66E-03 5.08E+01 -3.12E-01
NHW kg 0.00E+00 0.00E+00 0.00E+00 4.70E-01 1.43E-01 3.99E-01 -6.49E+00
RW kg 0.00E+00 0.00E+00 0.00E+00 5.01E-05 1.54E-05 8.11E-05 -4.52E-04
HW Hazardous waste disposed; NHW Non hazardous waste disposed; RW Radioactive waste disposed
End of life- Output flow with alu clad
Parameter Unit A1-A3 A4 A5 B1 B2 B3 B4 B5
CR kg 0.00E+00 0.00E+00 0.00E+00 0.00E+00 0.00E+00 0.00E+00 0.00E+00 0.00E+00
MR kg 4.12E-01 0.00E+00 1.30E-01 0.00E+00 5.07E-03 0.00E+00 0.00E+00 0.00E+00
MER kg 0.00E+00 0.00E+00 3.10E+00 0.00E+00 0.00E+00 0.00E+00 0.00E+00 0.00E+00
EEE MJ 9.61E+00 0.00E+00 0.00E+00 0.00E+00 0.00E+00 0.00E+00 0.00E+00 0.00E+00
ETE MJ 9.87E+01 0.00E+00 0.00E+00 0.00E+00 0.00E+00 0.00E+00 0.00E+00 0.00E+00
End of life- Output flow with alu clad
Parameter Unit B6 B7 C1 C2 C3 C4 D
CR kg 0.00E+00 0.00E+00 0.00E+00 0.00E+00 0.00E+00 0.00E+00 0.00E+00
MR kg 0.00E+00 0.00E+00 0.00E+00 0.00E+00 2.02E+00 0.00E+00 -2.21E+00
MER kg 0.00E+00 0.00E+00 0.00E+00 0.00E+00 0.00E+00 0.00E+00 0.00E+00
EEE MJ 0.00E+00 0.00E+00 0.00E+00 0.00E+00 2.91E+01 0.00E+00 -2.67E+01
ETE MJ 0.00E+00 0.00E+00 0.00E+00 0.00E+00 2.02E+02 0.00E+00 -2.52E+02
CR Components for reuse; MR Materials for recycling; MER Materials for energy recovery; EEE Exported electric energy; ETE Exported thermal
energy
Reading example: 9,0 E-03 = 9,0*10-3 = 0,009
NEPD-3451-2058-EN NTech inward opening windows 105/80 – ND, NS, NB (with aluminium cladding)
7/9
Norwegian additional requirements
Greenhouse gas emissions from the use of electricity in the production phase
National (Norway) market with low-voltage, including production of transmission lines and grid losses, has been used for electricity in
the production process (A3).
Data source Quantity Unit
Ecoinvent v3.7 (september 2020) 23 gram CO -ekv./kWh
2
Hazardous substances
The product contains no substances from REACH Candidate List or the Norwegian Priority List
The product contains substances below 0.1% by weight on the REACH Candidate List
The product contains substances from REACH Candidate List or the Norwegian Priority List, see table under Specific
Norwegian requirements.
The product does not contain any substances on the REACH Candidate List or the Norwegian Priority List. The product can be
characterized as hazardous waste (according to the Waste Shift, Appendix III), see table under Specific Norwegian
requirements.
Transport
Transport from production site to construction site according to scenario in A4: 250+50 km
Indoor air quality
The product has not been tested for emissions to indoor environments.
Carbon footprint
To increase the transparency of the climate impacts, the GWP indicator has been divided into sub-indicators:
GWP-IOBC Climate impacts calculated according to instant oxidation principle
GWP-BCIP Climate impacts calculated from the net impacts of sequestration and emission of biogenic carbon
Climate impact with alu clad
Parameter Unit A1-A3 A4 A5 B1 B2 B3 B4 B5
GWP-IOBC kg CO -ekv 1.32E+02 2.24E+00 0.00E+00 0.00E+00 6.60E+01 0.00E+00 0.00E+00 0.00E+00
2
GWP-BCIP kg CO -ekv -3.10E+01 0.00E+00 4.55E+00 0.00E+00 0.00E+00 0.00E+00 0.00E+00 0.00E+00
2
GWP kg CO -ekv 1.01E+02 2.24E+00 4.55E+00 0.00E+00 6.60E+01 0.00E+00 0.00E+00 0.00E+00
2
Climate impact with alu clad
Parameter Unit B6 B7 C1 C2 C3 C4 D
GWP-IOBC kg CO -ekv 0.00E+00 0.00E+00 0.00E+00 4.74E-01 7.68E+00 5.34E-01 -3.51E+01
2
GWP-BCIP kg CO -ekv 0.00E+00 0.00E+00 0.00E+00 0.00E+00 2.64E+01 0.00E+00 0.00E+00
2
GWP kg CO -ekv 0.00E+00 0.00E+00 0.00E+00 4.74E-01 3.41E+01 5.34E-01 -3.51E+01
2
Additional information
For the products with different sizes from the declared unit, the environmental impacts must be converted by using a conversion factor.
The Norwegian EPD Foundation has published instructions on how to interpret EPDs for windows on its website (www.epd-norge.no)
where different calculation methods have been stated. (Document: Bruksanvisninger i hvordan tolke EPD'er – Vinduer)
NEPD-3451-2058-EN NTech inward opening windows 105/80 – ND, NS, NB (with aluminium cladding)
8/9
Bibliografi
NS-EN ISO 14025:2010 Miljømerker og deklarasjoner - Miljødeklarasjoner type III - Prinsipper og prosedyrer.
NS-EN ISO 14044:2006 Miljøstyring - Livsløpsvurderinger - Krav og retningslinjer
NS-EN 15804:2012+A1:2013 Bærekraftig byggverk - Miljødeklarasjoner - Grunnleggende produktkategoriregler for
byggevarer
ISO 21930:2007 Sustainability in building construction - Environmental declaration of building products
Modaresi, R. 2020 LCA-report for Nordan LCA-report nr. 325039-3 from Norwegian Institute of Wood
Technology, Oslo, Norway.
NPCR014 (04/2019) Product category rules for windows and doors, rev3, April 2019
NS-EN 16485:2014 Tømmer og skurlast - Miljødeklarasjoner - Produktkategoriregler for tre og trebaserte produkter
til bruk i byggverk
NS-EN 16449:2014 Tre og trebaserte produkter - Beregning av biogent karboninnhold i tre og omdanning til
karbondioksid
Ecoinvent v3.0-3.7 Ecoinvent database version 3.0-3.7 Centre for Life Cycle Inventories.
Statistisk sentralbyrå Tabell 04727: Fjernvarmebalansen, 2015
Statistisk sentralbyrå Tabell 09469: Nettoproduksjon av fjernvarme, 2015
NEPD-307-179-NO EPD for skurlast av gran eller furu. Treindustrien
Bruksanvisninger i hvordan tolke EPD'er – Vinduer. https://www.epd-norge.no [in Norwegian]
Program operator and publisher Tlf: +47 23 08 80 00
The Norwegian EPD Foundation
Postboks 5250 Majorstuen, 0303 Oslo e-post: post@epd-norge.no
Norway web www.epd-norge.no
Owner of the declaration Tlf: +47 51 40 40 00
NorDan AS
Stasjonsveien 46, N-4460 Moi e-post: firmapost@nordan.no
Norway
web www.nordan.no
Author of the Life Cycle Assessment Tlf: +47 98 85 33 33
Roja Modaresi
Norsk Treteknisk Instiutt e-post: firmapost@treteknisk.no
Postboks 113 Blindern, 0314 Oslo, Norway web www.treteknisk.no
NEPD-3451-2058-EN NTech inward opening windows 105/80 – ND, NS, NB (with aluminium cladding)
9/9
EPD for the best
environmental
decision
www.epd-norge.no
The Norwegian EPD foundation
EPD for the best environmental decision
12
