Environmental product declaration
in accordance with ISO 14025 and EN 15804+A2
giroflex 313
Owner of the declaration: Program operator:
Flokk AS The Norwegian EPD Foundation
Product: Declaration number:
giroflex 313
Registration number:
Declared unit:
1 pcs Issue date:
This declaration is based on Product Category Rules: Valid to:
CEN Standard EN 15804:2012+A2:2019 serves as core
EPD software:
PCR
LCAno EPD generator ID: 573515
The Norwegian EPD Foundation NPCR 026:2022 Part B for Furniture
1 / 13
General information
Product Owner of the declaration:
giroflex 313 Flokk AS
Contact person: Atle Thiis-Messel
Phone: 0047 98 25 68 30
e-mail: atle.messel@flokk.com
Program operator: Manufacturer:
The Norwegian EPD Foundation Flokk AS
Post Box 5250 Majorstuen, 0303 Oslo, Norway Drammensveien 145,
Phone: +47 977 22 020 0277 Oslo, Norway
web: www.epd-norge.no
Declaration number: Place of production:
Flokk - Turek
ul. Górnicza 8
62-700 Turek, Poland
This declaration is based on Product Category Rules: Management system:
CEN Standard EN 15804:2012+A2:2019 serves as core PCR ISO 14001, ISO 9001.
NPCR 026:2022 Part B for Furniture
Statement of liability: Organisation no:
The owner of the declaration shall be liable for the underlying No 928 902 749
information and evidence. EPD Norway shall not be liable with respect
to manufacturer information, life cycle assessment data and
evidences.​
Declared unit: Issue date:
1 pcs giroflex 313
Declared unit (cradle to gate) with option: Valid to:
A1-A3,A4,A5,B2,B3,B4,C1,C2,C3,C4,D
Year of study:
2023
Functional unit: Comparability:
giroflex 313-4039 with ALU armrests fixed and softpads, upholstered EPD of construction products may not be comparable if they not
seat in Xtreme fabric from Camira, and mesh backrest in Runner from comply with EN 15804 and seen in a building context.
Gabriel - including large box packaging.
General information on verification of EPD from EPD tools: Development and verification of EPD:
Independent verification of data, other environmental information The declaration is created using EPD tool lca.tools ver EPD2022.03,
and the declaration according to ISO 14025:2010, § 8.1.3 and § 8.1.4. developed by LCA.no. The EPD tool is integrated in the company's
Verification of each EPD is made according to EPD-Norway’s management system, and has been approved by EPD Norway.
guidelines for verification and approval requiring that tools are i)
integrated into the company's environmental management system, ii) Developer of EPD: Damian Bakowski
the procedures for use of the EPD tool are approved by EPD-Norway,
Reviewer of company-specific input data and EPD: Monika Kuczynska
and iii) the process is reviewed annually by an independent third
party verifier. See Appendix G of EPD-Norway's General Programme
Instructions for further information on EPD tools
Verification of EPD tool: Approved:
Independent third party verification of the EPD tool, background data
and test-EPD in accordance with EPDNorway's procedures and
guidelines for verification and approval of EPD tools.
Third party verifier:
Elisabet Amat, GREENIZE projects
(no signature required)
2 / 13
Product
Product description:
Maximum comfort, intuitive self-adjustment, enhanced sitting. Today’s working world is fluid. Boundaries are blurring, interfaces merging, and
systems are losing their clear definition. We have created the giroflex 313 with these developments in mind. Based on a design platform that is
reduced to the bare essentials, the chair is ideal for both desk work and conferences. Where multiple people use the same chair, the giroflex 313
offers automatic self-adjustment while maintaining synchronisation. Our specially developed Balance Move System ensures the right results every
time. The seat and back align perfectly with the user’s body weight. The only parameters requiring manual adjustment are the seat hight and the
locking mechanism when the chair is in an upright position.
Product specification
The model studied in detail in this declaration is the giroflex 313 with ALU armrests fixed and softpads, upholstered seat in Xtreme fabric from
Camira, and mesh backrest in Runner from Gabriel - including large box packaging. The key environmental indicators for the other models and
options of the giroflex 313 are presented on a table page 12 of this declaration.
Recycled
Recycled share in share in
Materials kg %
material (kg) material
(%)
Plastic - Nylon (PA) 1,66 13,30 0,00 0,00
Plastic - Polyethylene
0,01 0,05 0,00 0,00
(HDPE)
Plastic -
Polyoxymethylene 0,09 0,76 0,00 0,00
(POM)
Plastic -
0,85 6,85 0,00 0,00
Polypropylene (PP)
Plastic - Polyurethane
0,60 4,81 0,00 0,00
(PUR)
Powder coating 0,05 0,36 0,00 0,00
Reinforcement 0,28 2,25 0,00 0,00
Rubber, synthetic 0,06 0,47 0,00 0,00
Textile - Felt 0,00 0,00 0,00 0,00
Textile - Polyester (PE) 0,51 4,08 0,38 74,02
Metal - Aluminium 6,34 50,84 6,34 100,00
Metal - Brass 0,07 0,57 0,01 17,71
Metal - Steel 1,95 15,62 0,31 16,17
Others 0,00 0,04 0,00 1,24
Total 12,47 100,00 7,04
Recycled
Recycled share in share in
Packaging kg %
material (kg) material
(%)
Packaging - Paper 0,02 0,40 0,01 34,31
Packaging - Plastic 0,23 5,83 0,00 0,00
Packaging - Plastic
0,00 0,01 0,00 0,00
straps
Recycled cardboard 3,76 93,76 3,76 100,00
Total incl. packaging 16,48 100,00 10,81
Technical data:
giroflex 313 – Swivel chair: available with upholstered back rest and structured back shell, or 3D spacer fabric in a wide range of colours. Manual
back rest locking mechanism in upright position included as standard. Seat upholstered with high-quality textile or leather covering. Height
adjustable column chromiumplated on request. Optional fixed plastic arm rests. Powder-coated five-arm base, seat and backframe, with optional
polished finish. Castors in black. Antistatic finish available on request.
giroflex 313 – Conference chair: available with upholstered back rest and structured back shell, or 3D spacer fabric in a wide range of colours. No
back rest locking mechanism in upright position. Seat upholstered with high-quality textile or leather covering. Optional fixed plastic arm rests.
Column chromium-plated on request, optional height adjustment and auto return. Polished or powder-coated four-arm base, castors or glides.
Powder-coated seat and backframe with optional polished finish. Antistatic finish available on request.
Market:
Worldwide
Reference service life, product
5 years
Reference service life, building
LCA: Calculation rules
3 / 13
Declared unit:
1 pcs giroflex 313
Cut-off criteria:
All major raw materials and all the essential energy is included. The production processes for raw materials and energy flows with very small
amounts (less than 1%) are not included. These cut-off criteria do not apply for hazardous materials and substances.
Allocation:
The allocation is made in accordance with the provisions of EN 15804. Incoming energy and water and waste production in-house is allocated
equally among all products through mass allocation. Effects of primary production of recycled materials is allocated to the main product in which
the material was used. The recycling process and transportation of the material is allocated to this analysis.
Data quality:
Specific data for the product composition are provided by the manufacturer. They represent the production of the declared product and were
collected for EPD development in the year of study. Background data is based on registered EPDs according to EN 15804, Ostfold Research
databases, ecoinvent and other LCA databases. The data quality of the raw materials in A1 is presented in the table below.​
Materials Source Data quality Year
Metal - Aluminium ecoinvent 3.6 Database 2019
Metal - Brass ecoinvent 3.6 Database 2019
Metal - Steel ecoinvent 3.6 Database 2019
Metal - Steel Modified ecoinvent 3.6 Database 2019
Others ecoinvent 3.6 Database 2019
Packaging - Paper ecoinvent 3.6 Database 2019
Packaging - Plastic ecoinvent 3.6 Database 2019
Packaging - Plastic straps ecoinvent 3.6 Database 2019
Plastic - Nylon (PA) ecoinvent 3.6 Database 2019
Plastic - Polyethylene (HDPE) ecoinvent 3.6 Database 2019
Plastic - Polyoxymethylene (POM) ecoinvent 3.6 Database 2019
Plastic - Polypropylene (PP) ecoinvent 3.6 Database 2019
Plastic - Polyurethane (PUR) ecoinvent 3.6 Database 2019
Powder coating Ecoinvent 3.6 Database 2019
Recycled cardboard Modified ecoinvent 3.6 Database 2019
Reinforcement ecoinvent 3.6 Database 2019
Rubber, synthetic ecoinvent 3.6 Database 2019
Textile - Felt Modified ecoinvent 3.6 Database 2019
Textile - Polyester (PE) ecoinvent 3.6 Database 2019
Textile - Polyester (PE) Modified ecoinvent 3.6 Database 2019
4 / 13
System boundaries (X=included, MND=module not declared, MNR=module not relevant)
Construction Beyond the system
Product stage Use stage End of life stage
installation stage boundaries
A1 A2 A3 A4 A5 B1 B2 B3 B4 B5 B6 B7 C1 C2 C3 C4 D
X X X X X MND X X X MND MND MND X X X X X
System boundary:
Additional technical information:
waR slairetam tropsnarT gnirutcafunaM tropsnarT ylbmessA e​sU ecnanetniaM riapeR tnemecalpeR tnemhsibrufeR lanoitarepO ygrene esu lanoitarepO esu retaw -eD noitcurtsnoc noitilomed tropsnarT etsaW gnissecorp lasopsiD -yrevoceR-esueR laitnetop-gnilcyceR
5 / 13
LCA: Scenarios and additional technical information
The following information describe the scenarios in the different modules of the EPD.
Capacity utilisation Value
Transport from production place to user (A4) Distance (km) Fuel/Energy Consumption Unit
(incl. return) % (Liter/tonne)
Truck, over 32 tonnes, EURO 5 (km) 53,3 % 1000 0,023 l/tkm 23,00
Assembly (A5) Unit Value
Waste, packaging, plastic film (LDPE), to average
kg 0,23
treatment - A5 (kg)
Waste, packaging, PET straps, to average
kg 0,00
treatment - A5 (kg)
Waste, packaging, paper printed, to average
kg 0,02
treatment (kg)
Waste, packaging, cardboard, 100 % recycled, to
kg 3,76
average treatment (kg)
Maintenance (B2) Unit Value
Water, tap water (m3) m3/DU 0,78
Electricity, European average (kWh) kWh/DU 10,53
Electricity, World average (kWh) kWh/DU 1,17
Repair (B3) Unit Value
Electricity, European average (kWh) kWh/DU 0,50
Electricity, World average (kWh) kWh/DU 0,06
Capacity utilisation Value
Transport to waste processing (C2) Distance (km) Fuel/Energy Consumption Unit
(incl. return) % (Liter/tonne)
Truck, 16-32 tonnes, EURO 5 (km) 36,7 % 85 0,044 l/tkm 3,74
Waste processing (C3) Unit Value
Waste treatment per kg Textile, incineration with
kg 0,51
fly ash extraction (kg)
Waste, materials to recycling (kg) kg 1,33
Waste treatment per kg Scrap steel, incineration
kg 1,95
with fly ash extraction (kg)
Waste treatment per kg Polyurethane (PU),
kg 0,60
incineration (kg)
Waste treatment per kg Polypropylene (PP),
kg 0,85
incineration with fly ash extraction - C3 (kg)
Waste treatment per kg Plastics, Mixture,
kg 1,66
municipal incineration with fly ash extraction (kg)
Waste treatment per kg Scrap aluminium,
kg 6,34
incineration with fly ash extraction (kg)
Waste treatment per kg Scrap copper, incineration
kg 0,07
with fly ash extraction (kg)
Waste treatment per kg Non-hazardous waste,
kg 0,33
incineration with fly ash extraction - C3 (kg)
Waste treatment per kg Polyoxymethylene (POM),
kg 0,09
incineration with fly ash extraction (kg) - CH - C3
Waste treatment per kg Rubber, municipal
kg 0,06
incineration with fly ash extraction (kg)
Waste treatment per kg Polyethylene, PE,
kg 0,01
incineration with fly ash extraction - C3 (kg)
6 / 13
Disposal (C4) Unit Value
Landfilling of ashes from incineration of Textile,
kg 0,03
soiled, process per kg ashes and residues (kg)
Landfilling of ashes and residues from
kg 1,29
incineration of Scrap steel (kg)
Landfilling of ashes from incineration of
Polyurethane (PU), process per kg ashes and kg 0,02
residues - C4 (kg)
Landfilling of ashes from incineration of
Polypropylene, PP, process per kg ashes and kg 0,03
residues - C4 (kg)
Landfilling of ashes from incineration of Plastics,
Mixture, municipal incineration with fly ash
kg 0,06
extraction, process per kg ashes and residues - C4
(kg)
Landfilling of ashes and residues from
kg 5,68
incineration of Scrap aluminium (kg)
Landfilling of ashes and residues from
kg 0,06
incineration of Scrap copper (kg)
Landfilling of ashes from incineration of Non-
hazardous waste, process per kg ashes and kg 0,08
residues - C4 (kg)
Landfilling of ashes from incineration of
Polyoxymethylene (POM), process per kg ashes kg 0,00
and residues (kg) - CH - C4
Landfilling of ashes from incineration of Rubber,
kg 0,00
process per kg ashes and residues - C4 (kg)
Landfilling of ashes from incineration of
Polyethylene, PE, process per kg ashes and kg 0,00
residues - C4 (kg)
Benefits and loads beyond the system
Unit Value
boundaries (D)
Substitution of electricity, in Norway (MJ) MJ 5,62
Substitution of thermal energy, district heating, in
MJ 85,10
Norway (MJ)
Substitution of primary steel with net scrap (kg) kg 0,55
Substitution of primary Brass with net scrap (kg) kg 0,01
7 / 13
LCA: Results
The LCA results are presented below for the declared unit defined on page 2 of the EPD document.
Environmental impact
Indicator Unit A1-A3 A4 A5 B2 B3
GWP-total kg CO2 -eq 3,87E+01 1,50E+00 6,49E+00 5,67E+00 2,54E-01
GWP-fossil kg CO2 -eq 4,46E+01 1,50E+00 7,96E-02 5,62E+00 2,52E-01
GWP-biogenic kg CO2 -eq -5,96E+00 6,15E-04 6,41E+00 3,61E-02 1,62E-03
GWP-luluc kg CO2 -eq 4,58E-02 4,37E-04 2,16E-05 1,27E-02 5,74E-04
ODP kg CFC11 -eq 2,27E-06 3,46E-07 1,40E-08 4,39E-07 1,95E-08
AP mol H+ -eq 2,38E-01 6,30E-03 3,12E-04 3,22E-02 1,44E-03
EP-FreshWater kg P -eq 1,80E-03 1,14E-05 5,40E-07 5,47E-04 2,47E-05
EP-Marine kg N -eq 4,78E-02 1,89E-03 1,17E-04 4,31E-03 1,91E-04
EP-Terrestial mol N -eq 5,00E-01 2,09E-02 1,12E-03 5,22E-02 2,32E-03
POCP kg NMVOC -eq 1,58E-01 6,74E-03 3,25E-04 1,35E-02 5,94E-04
ADP-minerals&metals1 kg Sb-eq 2,83E-02 2,56E-05 1,59E-06 4,34E-05 1,69E-06
ADP-fossil1 MJ 6,32E+02 2,33E+01 9,31E-01 1,08E+02 4,87E+00
WDP1 m3 1,35E+04 1,79E+01 1,35E+00 1,51E+03 6,70E+01
Indicator Unit B4 C1 C2 C3 C4 D
GWP-total kg CO2 -eq 0 0 2,34E-01 9,68E+00 7,97E-02 -1,15E+00
GWP-fossil kg CO2 -eq 0 0 2,34E-01 8,93E+00 7,96E-02 -1,13E+00
GWP-biogenic kg CO2 -eq 0 0 9,53E-05 7,45E-01 6,25E-05 -1,50E-03
GWP-luluc kg CO2 -eq 0 0 8,17E-05 5,47E-05 2,39E-05 -1,73E-02
ODP kg CFC11 -eq 0 0 5,33E-08 2,99E-08 2,45E-08 -3,59E-02
AP mol H+ -eq 0 0 9,55E-04 3,51E-03 5,61E-04 -9,60E-03
EP-FreshWater kg P -eq 0 0 1,83E-06 3,33E-06 7,96E-07 -1,01E-04
EP-Marine kg N -eq 0 0 2,83E-04 1,76E-03 2,00E-04 -2,08E-03
EP-Terrestial mol N -eq 0 0 3,13E-03 1,78E-02 2,21E-03 -2,26E-02
POCP kg NMVOC -eq 0 0 9,59E-04 4,33E-03 6,37E-04 -7,50E-03
ADP-minerals&metals1 kg Sb-eq 0 0 6,33E-06 1,35E-06 1,37E-06 -1,77E-04
ADP-fossil1 MJ 0 0 3,52E+00 2,12E+00 1,81E+00 -1,25E+01
WDP1 m3 0 0 3,36E+00 5,46E+00 3,62E+00 -5,66E+01
GWP-total = Global Warming Potential total; GWP-fossil = Global Warming Potential fossil fuels; GWP-biogenic = Global Warming Potential biogenic; GWP-luluc =
Global Warming Potential land use and land use change; ODP = Depletion potential of the stratospheric ozone layer; AP = Acidification potential, Accumulated
Exceedance; EP-freshwater = Eutrophication potential, fraction of nutrients reaching freshwater end compartment: EP-marine = Eutrophication potential, fraction of
nutrients reaching marine end compartment; EP-terrestrial = Eutrophication potential, Accumulated Exceedance; POCP = Formation potential of tropospheric ozone;
ADP-minerals&metals = Abiotic depletion potential for non-fossil resources; ADP-fossil = Abiotic depletion for fossil resources potential; WDP = Water (user)
deprivation potential, deprivation-weighted water consumption
"Reading example: 9,0 E-03 = 9,0*10-3 = 0,009"
*INA Indicator Not Assessed
1. The results of this environmental impact indicator shall be used with care as the uncertainties on these results are high or as there is limited experienced with the
indicator
Remarks to environmental impacts
8 / 13
Additional environmental impact indicators
Indicator Unit A1-A3 A4 A5 B2 B3
PM Disease incidence 2,22E-06 1,32E-07 4,68E-09 1,14E-07 4,75E-09
IRP2 kgBq U235 -eq 1,22E+00 1,02E-01 4,00E-03 8,90E-01 4,03E-02
ETP-fw1 CTUe 1,52E+03 1,70E+01 1,21E+00 8,66E+01 3,84E+00
HTP-c1 CTUh 5,82E-08 0,00E+00 3,50E-11 2,79E-09 9,70E-11
HTP-nc1 CTUh 1,08E-06 1,65E-08 1,50E-09 8,81E-08 3,37E-09
SQP1 dimensionless 1,68E+02 2,67E+01 7,07E-01 2,53E+01 1,13E+00
Indicator Unit B4 C1 C2 C3 C4 D
PM Disease incidence 0 0 1,68E-08 2,51E-08 1,03E-08 -3,02E-07
IRP2 kgBq U235 -eq 0 0 1,54E-02 4,57E-03 7,29E-03 -4,42E-02
ETP-fw1 CTUe 0 0 2,59E+00 4,82E+01 1,08E+00 -9,65E+01
HTP-c1 CTUh 0 0 0,00E+00 6,74E-10 3,80E-11 -3,98E-09
HTP-nc1 CTUh 0 0 2,80E-09 2,22E-08 1,04E-09 -2,54E-09
SQP1 dimensionless 0 0 2,43E+00 3,37E-01 3,93E+00 -4,79E+01
PM = Particulate Matter emissions; IRP = Ionizing radiation – human health; ETP-fw = Eco toxicity – freshwater; HTP-c = Human toxicity – cancer effects; HTP-nc =
Human toxicity – non cancer effects; SQP = Soil Quality (dimensionless)
"Reading example: 9,0 E-03 = 9,0*10-3 = 0,009"
*INA Indicator Not Assessed
1. The results of this environmental impact indicator shall be used with care as the uncertainties on these results are high or as there is limited experienced with the
indicator
2. This impact category deals mainly with the eventual impact of low dose ionizing radiation on human health of the nuclear fuel cycle. It does not consider effects due
to possible nuclear accidents, occupational exposure nor due to radioactive waste disposal in underground facilities. Potential ionizing radiation from the soil, from
radon and from some construction materials is also not measured by this indicator.
9 / 13
Resource use
Indicator Unit A1-A3 A4 A5 B2 B3
PERE MJ 1,12E+02 2,93E-01 1,60E-02 1,99E+01 9,05E-01
PERM MJ 2,22E+01 0,00E+00 -2,22E+01 0,00E+00 0,00E+00
PERT MJ 1,34E+02 2,93E-01 -2,22E+01 1,99E+01 9,05E-01
PENRE MJ 4,96E+02 2,33E+01 9,31E-01 1,08E+02 4,88E+00
PENRM MJ 1,37E+02 0,00E+00 -9,94E+00 0,00E+00 0,00E+00
PENRT MJ 6,33E+02 2,33E+01 -9,01E+00 1,08E+02 4,88E+00
SM kg 1,08E+01 0,00E+00 0,00E+00 0,00E+00 0,00E+00
RSF MJ 9,24E-01 1,03E-02 5,17E-04 1,38E+00 6,27E-02
NRSF MJ 2,11E-01 3,44E-02 2,06E-03 3,70E-01 1,51E-02
FW m3 5,84E-01 2,65E-03 4,44E-04 8,69E-01 3,99E-03
Indicator Unit B4 C1 C2 C3 C4 D
PERE MJ 0 0 4,97E-02 8,94E-02 3,39E-02 -4,41E+01
PERM MJ 0 0 0,00E+00 0,00E+00 0,00E+00 0,00E+00
PERT MJ 0 0 4,97E-02 8,94E-02 3,39E-02 -4,41E+01
PENRE MJ 0 0 3,52E+00 2,16E+00 1,81E+00 -1,25E+01
PENRM MJ 0 0 0,00E+00 -1,27E+02 0,00E+00 0,00E+00
PENRT MJ 0 0 3,52E+00 -1,25E+02 1,81E+00 -1,25E+01
SM kg 0 0 0,00E+00 0,00E+00 0,00E+00 -2,04E-03
RSF MJ 0 0 1,78E-03 2,03E-03 8,97E-04 1,37E-02
NRSF MJ 0 0 6,35E-03 0,00E+00 3,83E-02 -1,95E+00
FW m3 0 0 3,71E-04 8,43E-03 1,64E-03 -5,44E-02
PERE = Use of renewable primary energy excluding renewable primary energy resources used as raw materials; PERM = Use of renewable primary energy resources used
as raw materials; PERT = Total use of renewable primary energy resources; PENRE = Use of non renewable primary energy excluding non-renewable primary energy
resources used as raw materials; PENRM = Use of non renewable primary energy resources used as raw materials; PENRT = Total use of non renewable primary energy
resources; SM = Use of secondary materials; RSF = Use of renewable secondary fuels; NRSF = Use of non-renewable secondary fuels; FW = Net use of fresh water
"Reading example: 9,0 E-03 = 9,0*10-3 = 0,009"
*INA Indicator Not Assessed
10 / 13
End of life - Waste
Indicator Unit A1-A3 A4 A5 B2 B3
HWD kg 9,32E-01 1,28E-03 0,00E+00 1,87E-02 8,39E-04
NHWD kg 6,58E+00 2,03E+00 4,01E+00 4,24E-01 1,73E-02
RWD kg 1,18E-03 1,59E-04 0,00E+00 7,21E-04 3,26E-05
Indicator Unit B4 C1 C2 C3 C4 D
HWD kg 0 0 1,80E-04 0,00E+00 7,13E+00 -3,75E-03
NHWD kg 0 0 1,68E-01 3,26E-01 8,53E-02 -4,24E-01
RWD kg 0 0 2,40E-05 0,00E+00 1,13E-05 -3,63E-05
HWD = Hazardous waste disposed; NHWD = Non-hazardous waste disposed; RWD = Radioactive waste disposed
"Reading example: 9,0 E-03 = 9,0*10-3 = 0,009"
*INA Indicator Not Assessed
End of life - Output flow
Indicator Unit A1-A3 A4 A5 B2 B3
CRU kg 0,00E+00 0,00E+00 0,00E+00 0,00E+00 0,00E+00
MFR kg 8,33E-01 0,00E+00 3,63E+00 0,00E+00 0,00E+00
MER kg 7,87E-06 0,00E+00 1,14E-03 0,00E+00 0,00E+00
EEE MJ 4,60E-01 0,00E+00 2,16E-01 0,00E+00 0,00E+00
EET MJ 6,97E+00 0,00E+00 3,27E+00 0,00E+00 0,00E+00
Indicator Unit B4 C1 C2 C3 C4 D
CRU kg 0 0 0,00E+00 0,00E+00 0,00E+00 0,00E+00
MFR kg 0 0 0,00E+00 1,33E+00 0,00E+00 -2,75E-04
MER kg 0 0 0,00E+00 1,25E+01 0,00E+00 -3,31E-05
EEE MJ 0 0 0,00E+00 5,59E+00 0,00E+00 -2,09E-04
EET MJ 0 0 0,00E+00 8,46E+01 0,00E+00 -3,16E-03
CRU = Components for re-use; MFR = Materials for recycling; MER = Materials for energy recovery; EEE = Exported energy electrical; EET = Exported energy thermal
"Reading example: 9,0 E-03 = 9,0*10-3 = 0,009"
*INA Indicator Not Assessed
Biogenic Carbon Content
Indicator Unit At the factory gate
Biogenic carbon content in product kg C 0,00E+00
Biogenic carbon content in accompanying packaging kg C 1,75E+00
Note: 1 kg biogenic carbon is equivalent to 44/12 kg CO2
11 / 13
Additional requirements
Greenhouse gas emissions from the use of electricity in the manufacturing phase
National production mix from import, low voltage (production of transmission lines, in addition to direct emissions and losses in grid) of applied
electricity for the manufacturing process (A3).
Electricity mix Source Amount Unit
Electricity, high voltage, hydro (kWh) - PL ecoinvent 3.6 4,02 g CO2-eq/kWh
Dangerous substances
The product contains no substances given by the REACH Candidate list.
Indoor environment
Greenguard Gold.
Additional Environmental Information
Key Environmental Indicators
Key environmental indicators Unit A1-A3 A4 A1-C4 A1-D
GWPtotal kg CO2 -eq 38,71 1,50 62,61 61,46
Total energy consumption MJ 608,71 23,65 776,82 718,34
Amount of recycled materials % 65,54
Additional environmental impact indicators required in NPCR Part A for construction products
Indicator Unit A1-A3 A4 A5 B2 B3
GWPIOBC kg CO2 -eq 4,47E+01 1,50E+00 7,97E-02 5,99E+00 2,69E-01
Indicator Unit B4 C1 C2 C3 C4 D
GWPIOBC kg CO2 -eq 0 0 2,34E-01 9,41E+00 8,67E-02 -1,44E+00
GWP-IOBC: Global warming potential calculated according to the principle of instantaneous oxidation. In order to increase the transparency of biogenic carbon
contribution to climate impact, the indicator GWP-IOBC is required as it declares climate impacts calculated according to the principle of instantaneous oxidation.
GWP-IOBC is also referred to as GWP-GHG in context to Swedish public procurement legislation.
Variants and Options
Key environmental indicators (A1-A3) for variants of this EPD
Weight GWPtotal (kg Total energy Amount of recycled
Variants
(kg) CO2 -eq) consumption (MJ) materials (%)
giroflex 313-4039 - Swivel chair w/o accessories, Backrest Mesh (Runner/Gabriel), Seat
11,11 39,14 472,53 52,26
upholstered (Xtreme/Camira) - No Packaging
giroflex 313-4539 - Swivel chair w/o accessories, Backrest and seat upholstered
12,41 44,35 555,60 49,46
(Xtreme/Camira) - No Packaging
giroflex 313-4018 - Conference chair w/o accessories, Backrest Mesh (Runner/Gabriel), Seat
10,33 38,23 464,75 51,88
upholstered (Xtreme/Camira) - No Packaging
giroflex 313-4518 - Conference chair w/o accessories, Backrest and seat upholstered
11,64 43,44 547,82 48,94
(Xtreme/Camira) - No Packaging
Key environmental indicators (A1-A3) for options for this EPD
Options Weight (kg)GWPtotal (kg CO2 -eq) Total energy consumption (MJ) Amount of recycled materials (%)
giroflex 313 - Armrest fixed , plastic 0,72 2,12 42,01 5,38
giroflex 313 - Armrest fixed , aluminium, softpad 1,37 1,58 22,50 90,73
giroflex 313 - Footring 2,12 3,55 47,30 68,13
giroflex 313 - Packaging 1 (Only foil, fully assembled) 0,17 0,48 8,14 3,22
giroflex 313 - Packaging 2 (Small box, partially assembled) 3,83 -1,78 109,65 92,93
giroflex 313 - Packaging 3 (Large box, fully assembled) 4,01 -2,00 113,69 93,90
12 / 13
Bibliography
ISO 14025:2010 Environmental labels and declarations - Type III environmental declarations - Principles and procedures.
ISO 14044:2006 Environmental management - Life cycle assessment - Requirements and guidelines.
EN 15804:2012+A2:2019 Environmental product declaration - Core rules for the product category of construction products.
ISO 21930:2017 Sustainability in buildings and civil engineering works - Core rules for environmental product declarations of construction
products.
ecoinvent v3, Allocation, cut-off by classification, Swiss Centre of Life Cycle Inventories.
Iversen et al., (2021) eEPD v2021.09 Background information for EPD generator tool system verification, LCA.no Report number: 07.21
Ruud et al., (2023) EPD generator for NPCR026 Part B for Furniture - Background information for EPD generator application and LCA data,
LCA.no report number 01.23
NPCR Part A: Construction products and services. Ver. 2.0. March 2021, EPD-Norge.
NPCR 026 Part B for Furniture. Ver. 2.0 March 2022, EPD-Norge.
Program operator and publisher Phone: +47 977 22 020
The Norwegian EPD Foundation e-mail: post@epd-norge.no
Post Box 5250 Majorstuen, 0303 Oslo, Norway web: www.epd-norge.no
Owner of the declaration: Phone: 0047 98 25 68 30
Flokk AS e-mail: atle.messel@flokk.com
Drammensveien 145,, 0277 Oslo web: https://www.flokk.com
Author of the Life Cycle Assessment Phone: +47 916 50 916
LCA.no AS e-mail: post@lca.no
Dokka 6A, 1671 Kråkerøy web: www.lca.no
Developer of EPD generator Phone: +47 916 50 916
LCA.no AS e-mail: post@lca.no
Dokka 6A, 1671 Kråkerøy web: www.lca.no
ECO Platform web: www.eco-platform.org
ECO Portal web: ECO Portal
13 / 13
