Environmental product declaration
in accordance with ISO 14025 and EN 15804+A2
Jotun Essence Easy Primer, P.T. Jotun Indonesia
Owner of the declaration: Program operator:
Jotun A/S The Norwegian EPD Foundation
Product: Declaration number:
Jotun Essence Easy Primer, P.T. Jotun Indonesia NEPD-5220-4546-EN
Declared unit: Registration number:
1 kg NEPD-5220-4546-EN
This declaration is based on Product Category Rules: Issue date:
CEN Standard EN 15804:2012+A2:2019 serves as core 23.10.2023
PCR
The Norwegian EPD Foundation IBU PCR Part B for coatings with organic binders Valid to:
23.10.2028
ver-061123
EPD Software:
LCA.no EPD generator ID: 68903
1 / 12
General information
Product Owner of the declaration:
Jotun Essence Easy Primer, P.T. Jotun Indonesia Jotun A/S
Contact person: Cleo Alves Otterbech
Phone: +47 33 45 70 00
e-mail: cleo.otterbech@jotun.no
Program operator: Manufacturer:
Post Box 5250 Majorstuen, 0303 Oslo, Norway P.T. Jotun Indonesia
The Norwegian EPD Foundation
Phone: +47 23 08 80 00
web: post@epd-norge.no
Declaration number: Place of production:
NEPD-5220-4546-EN P.T. Jotun Indonesia
Kawasan Industri MM2100, Jalan Irian III,Blok KK1 Cikarang Barat
17520 Bekasi, Indonesia
This declaration is based on Product Category Rules: Management system:
CEN Standard EN 15804:2012+A2:2019 serves as core PCR ISO 9001:2008 Certificate nr: 0044915-00, ISO 14001:2004
IBU PCR Part B for coatings with organic binders Certificate nr 0044914-00, ISO 45001: 2018 Certificate nr: 0098139
Statement of liability: Organisation no:
The owner of the declaration shall be liable for the underlying 923 248 579
information and evidence. EPD Norway shall not be liable with respect
to manufacturer information, life cycle assessment data and
evidences.​
Declared unit: Issue date:
1 kg Jotun Essence Easy Primer, P.T. Jotun Indonesia 23.10.2023
Declared unit with option: Valid to:
A1,A2,A3,A4,C1,C2,C3,C4,D 23.10.2028
Year of study:
2023
Functional unit: Comparability:
EPD of construction products may not be comparable if they not
comply with EN 15804 and seen in a building context.
General information on verification of EPD from EPD tools: Development and verification of EPD:
Independent verification of data, other environmental information The declaration is created using EPD tool lca.tools ver EPD2022.03,
and the declaration according to ISO 14025:2010, § 8.1.3 and § 8.1.4. developed by LCA.no. The EPD tool is integrated in the company's
Verification of each EPD is made according to EPD-Norway’s management system, and has been approved by EPD Norway.
guidelines for verification and approval requiring that tools are i) Approval number: NEPDT07
integrated into the company's environmental management system, ii)
the procedures for use of the EPD tool are approved by EPD-Norway, Developer of EPD: Joaquin Quezada
and iii) the process is reviewed annually by an independent third
Reviewer of company-specific input data and EPD:​ Cleo Alves
party verifier. See Appendix G of EPD-Norway's General Programme
Otterbech
Instructions for further information on EPD tools.
Verification Approved:
Independent third party verification of the EPD tool, background data
and test EPD in accordance with EPD Norway's procedures and
guidelines for verification and approval of EPD tools.
Håkon Hauan, CEO EPD-Norge
Third party verifier:
Anne Rønning - NORSUS
2 / 12
Product
Product description:
Jotun Essence Easy Primer is a modified acrylic water-based alkali-resistant primer that is easy to use and improves the performance of interior
topcoats.
The declared product features and benefits:
Good adhesion - Ensures good adhesion between concrete surface and topcoat to give lasting paint performance.
Alkali resistant - Resists alkali attack that causes discoloration and improves the performance and appearance of the paint.
Easy to Apply - Effortless application with smooth finish.
Formulation - Free from APEO and formaldehyde emissions, and heavy metals have not been used as active ingredients.
Low volatile organic compound (VOC).
Jotun Essence Easy Primer is recommended for interior application. It is suitable for new buildings, repainting and specifically on concrete,
masonry, plaster, brick work and soft board surfaces.
Product specification
For information on Green Building Standard credits, see subchapter "Additional technical information".
The material composition of the declared product is given below:
Materials Value Unit
Filler 25 - 50 %
Water 25 - 50 %
Binder 10 - 25 %
Titanium dioxide 3 - 5 %
Solvent 1 - 3 %
Additive 0.3 - 1 %
Pigment 0.1 - 0.3 %
Biocide 0 - 0.1 %
Technical data:
Density: 1.3 g/cm³
Solids by volume: 35 ± 2 volume%
Film thickness per coat:
Wet film thickness: 85 - 114 µm
Dry film thickness: 30 - 40 µm
Theoretical spreading rate: 11.6 - 8.8 m²/l
The most representative and worst case formulation produced at the manufacturing site is chosen for this EPD. For products with a selection of
colours, this will be the formulation with the highest content of titanium dioxide.
The product packaging is based on an average sized plastic packaging, including secondary packaging such as pallets and plastic wrapping.
For safety, health and environmental conditions, see the Safety Data Sheet for the declared product on www.jotun.com.
For information on technical data, application and use of the product, see the Technical Data Sheet for the declared product on www.jotun.com.
Market:
It covers the regional markets where the product is produced.
Reference service life, product
The reference service life of the product is highly dependent on the conditions of use.
Estimated service life, object
The coated object is not declared.
3 / 12
LCA: Calculation rules
Declared unit:
1 kg Jotun Essence Easy Primer, P.T. Jotun Indonesia
Cut-off criteria:
All major raw materials and all the essential energy is included. The production processes for raw materials and energy flows with very small
amounts (less than 1%) are not included. These cut-off criteria do not​ apply for hazardous materials and substances.
Allocation:
The allocation is made in accordance with the provisions of EN 15804. Incoming energy and water and waste production in-house is allocated
equally among all products through mass allocation. Effects of primary production of recycled materials is allocated to the main product in which
the material was used. The recycling process and transportation of the material is allocated to this analysis.
Data quality:
Specific data for the product composition are provided by the manufacturer. The data represent the production of the declared product and were
collected for EPD development in the year of study. Background data is based on EPDs according to EN 15804 and different LCA databases. The
data quality of the raw materials in A1 is presented in the table below.
Materials Source Data quality Year
Additives CEPE RM Database v3.0 Database 2016
Binders and Resins CEPE RM Database v3.0 Database 2016
Others CEPE RM Database v3.0 Database 2016
Pigments and Fillers CEPE RM Database v3.0 Database 2016
Solvent CEPE RM Database v3.0 Database 2016
Packaging ecoinvent 3.6 Database 2019
4 / 12
System boundaries (X=included, MND=module not declared, MNR=module not relevant)
Construction Beyond the system
Product stage Use stage End of life stage
installation stage boundaries
A1 A2 A3 A4 A5 B1 B2 B3 B4 B5 B6 B7 C1 C2 C3 C4 D
X X X X MND MND MND MND MND MND MND MND X X X X X
System boundary:
The flowchart in the figure below illustrates the system boundaries for the analysis, in accordance with the modular principle on EN 15804+A2. The
analysis is a cradle-to-gate (A1-A3) study with options, in addition to module A4, transport to market, modules C1-C4 and module D are included.
Additional technical information:
The declared product contributes to Green Building Standard credits by meeting the following specific requirements:
LEED®v4.1 (2020)/LEED®v4 (2013)
EQ credit: Low-emitting materials
-VOC content for Primers, Sealers and Undercoaters (100 g/l) (CARB(SCM)2020) and emission range between 0.5 and 5.0 mg/m³ (CDPH method
1.2).
MR credit: Building product disclosure and optimization
-Material Ingredients, Option 2: Material Ingredient Optimization, International Alternative Compliance Path - REACH optimization: Fully
inventoried chemical ingredients to 100 ppm and not containing substances on the REACH Authorization list – Annex XIV, the Restriction list –
Annex XVII and the SVHC candidate list.
-Environmental Product Declarations: Product-specific Type III EPD (ISO 14025;21930, EN 15804+A2) for P.T. Jotun Indonesia.
BREEAM® International v6.0 (2021)/BREEAM® International (2016)
-Hea 02: VOC emission (CDPH method 1.2 (2017)) and the VOC content for Primers (15 g/l).
-Mat 01: Product-specific Type III EPD (ISO 14025;21930, EN 15804+A2) for P.T. Jotun Indonesia.
Additional certificates and approvals may be available on request.
waR slairetam tropsnarT gnirutcafunaM tropsnarT ylbmessA e​sU ecnanetniaM riapeR tnemecalpeR tnemhsibrufeR lanoitarepO ygrene esu lanoitarepO esu retaw -eD noitcurtsnoc noitilomed tropsnarT etsaW gnissecorp lasopsiD -yrevoceR-esueR laitnetop-gnilcyceR
5 / 12
LCA: Scenarios and additional technical information
The following information describe the scenarios in the different modules of the EPD.
This is a cradle to gate (A1-A3) study with options, modules C1-C4, module D and additional module A4 transport to market has been included,
as described below.​
Module A4 includes the transport of 1 kg of the declared product with packaging from place of production to the market where the product is
sold. The calculation is based on average distances to distribution centers in the local market. The declared product is assumed to be transported
with the common type of truck used locally.​
Module C considers the end-of-life of the construction material. The calculations for module C are based on dried/cured paint. Solvents and water
are subtracted from the total coating mass due to the drying/curing processes occurring in modules A5 and B2. Similarly, packaging waste is
generated in module A5 and B2, thus it is not accounted for in module C.​
Module C1 is modelled with zero impact for the declared product. The coating is not removed from the substrate during decommissioning
process, therefore the impact is allocated to the coated object.​
Module C2 includes the transport of the paint waste to the closest disposal or waste treatment facility. It is assumed that the waste is transported
by truck with average characteristics listed in the Table. The transportation distance is set to 50 km.​
Module C3 is modelled with no waste paint processing.​
Module C4, paint waste is gathered as part of the substrate in construction materials. A typical disposal scenario for paint applied on that
substrate is landfill, therefore it is assumed that 100% of the paint waste is sent to landfill facilities.​
Module D. Recycling of applied paint is not a common practice, therefore the reuse, recovery and recycling potential is set to zero.
Capacity utilisation Value
Transport from production place to user (A4) Distance (km) Fuel/Energy Consumption Unit
(incl. return) % (Liter/tonne)
Truck World, over 32 tonnes, EURO 4 (km) 55,0 % 1523 0,023 l/tkm 35,03
De-construction demolition (C1) Unit Value
Energy use during decommissioning kWh/DU 0,00
Capacity utilisation Value
Transport to waste processing (C2) Distance (km) Fuel/Energy Consumption Unit
(incl. return) % (Liter/tonne)
Truck World, over 32 tonnes, EURO 4 (km) 55,0 % 50 0,023 l/tkm 1,15
Waste processing (C3) Unit Value
Waste treatment per kg Paint, municipal
kg/DU 0,00
incineration, World (kg)
Disposal (C4) Unit Value
Waste treatment per kg Paint, inert material
kg/DU 0,51
landfill, World (kg)
Benefits and loads beyond the system
Unit Value
boundaries (D)
Substitution of raw materials (kg) kg/DU 0,00
6 / 12
LCA: Results
The LCA results are presented below for the declared unit defined on page 2 of the EPD document.
Environmental impact
Indicator Unit A1 A2 A3 A4 C1 C2 C3 C4 D
GWP-total kg CO2 -eq 1,23E+00 2,06E-02 1,15E-01 1,55E-01 0,00E+00 2,37E-03 0,00E+00 9,92E-03 0,00E+00
GWP-fossil kg CO2 -eq 1,25E+00 2,06E-02 1,14E-01 1,55E-01 0,00E+00 2,37E-03 0,00E+00 9,91E-03 0,00E+00
GWP-biogenic kg CO2 -eq -1,58E-02 7,23E-06 5,73E-04 6,14E-05 0,00E+00 9,43E-07 0,00E+00 4,75E-06 0,00E+00
GWP-luluc kg CO2 -eq 1,90E-04 9,26E-06 2,51E-04 4,66E-05 0,00E+00 7,15E-07 0,00E+00 3,27E-06 0,00E+00
ODP kg CFC11 -eq 9,39E-08 4,55E-09 4,98E-09 3,49E-08 0,00E+00 5,36E-10 0,00E+00 2,75E-09 0,00E+00
AP mol H+ -eq 6,76E-03 3,20E-04 6,09E-04 7,94E-04 0,00E+00 1,22E-05 0,00E+00 5,50E-05 0,00E+00
EP-FreshWater kg P -eq 1,79E-04 1,47E-07 1,79E-05 1,39E-06 0,00E+00 2,13E-08 0,00E+00 8,68E-08 0,00E+00
EP-Marine kg N -eq 9,83E-04 8,43E-05 1,23E-04 2,65E-04 0,00E+00 4,07E-06 0,00E+00 1,75E-05 0,00E+00
EP-Terrestial mol N -eq 1,02E-02 9,37E-04 1,36E-03 2,93E-03 0,00E+00 4,49E-05 0,00E+00 1,94E-04 0,00E+00
POCP kg NMVOC -eq 3,87E-03 2,52E-04 3,60E-04 8,72E-04 0,00E+00 1,34E-05 0,00E+00 5,77E-05 0,00E+00
ADP-minerals&metals1 kg Sb -eq 4,70E-06 2,75E-07 2,97E-07 2,62E-06 0,00E+00 4,02E-08 0,00E+00 2,20E-07 0,00E+00
ADP-fossil1 MJ 2,38E+01 2,97E-01 1,19E+00 2,38E+00 0,00E+00 3,65E-02 0,00E+00 1,84E-01 0,00E+00
WDP1 m3 2,05E+01 8,96E-02 1,54E+00 8,42E-01 0,00E+00 1,29E-02 0,00E+00 1,27E-01 0,00E+00
GWP-total = Global Warming Potential total; GWP-fossil = Global Warming Potential fossil fuels; GWP-biogenic = Global Warming Potential biogenic; GWP-luluc =
Global Warming Potential land use and land use change; ODP = Depletion potential of the stratospheric ozone layer; AP = Acidification potential, Accumulated
Exceedance; EP-freshwater = Eutrophication potential, fraction of nutrients reaching freshwater end compartment: EP-marine = Eutrophication potential, fraction of
nutrients reaching marine end compartment; EP-terrestrial = Eutrophication potential, Accumulated Exceedance; POCP = Formation potential of tropospheric ozone;
ADP-minerals&metals = Abiotic depletion potential for non-fossil resources; ADP-fossil = Abiotic depletion for fossil resources potential; WDP = Water (user)
deprivation potential, deprivation-weighted water consumption
"Reading example: 9,0 E-03 = 9,0*10-3 = 0,009"
*INA Indicator Not Assessed
1. The results of this environmental impact indicator shall be used with care as the uncertainties on these results are high or as there is limited experienced with the
indicator
Remarks to environmental impacts
7 / 12
Additional environmental impact indicators
Indicator Unit A1 A2 A3 A4 C1 C2 C3 C4 D
PM Disease incidence 8,94E-08 1,10E-09 8,31E-09 1,33E-08 0,00E+00 2,04E-10 0,00E+00 1,02E-09 0,00E+00
IRP2 kgBq U235 -eq 9,89E+01 1,26E-03 9,43E-04 1,00E-02 0,00E+00 1,54E-04 0,00E+00 7,84E-04 0,00E+00
ETP-fw1 CTUe 7,00E+00 2,12E-01 5,27E-01 1,86E+00 0,00E+00 2,86E-02 0,00E+00 1,25E-01 0,00E+00
HTP-c1 CTUh 2,60E-09 0,00E+00 3,00E-11 0,00E+00 0,00E+00 0,00E+00 0,00E+00 1,00E-12 0,00E+00
HTP-nc1 CTUh 1,53E-07 1,36E-10 1,14E-09 1,66E-09 0,00E+00 2,60E-11 0,00E+00 1,20E-10 0,00E+00
SQP1 dimensionless 4,36E+00 2,36E-01 6,01E-02 2,69E+00 0,00E+00 4,13E-02 0,00E+00 2,29E-01 0,00E+00
PM = Particulate Matter emissions; IRP = Ionizing radiation – human health; ETP-fw = Eco toxicity – freshwater; HTP-c = Human toxicity – cancer effects; HTP-nc =
Human toxicity – non cancer effects; SQP = Potential Soil Quality Index (dimensionless)
"Reading example: 9,0 E-03 = 9,0*10-3 = 0,009"
*INA Indicator Not Assessed
1. The results of this environmental impact indicator shall be used with care as the uncertainties on these results are high or as there is limited experienced with the
indicator
2. This impact category deals mainly with the eventual impact of low dose ionizing radiation on human health of the nuclear fuel cycle. It does not consider effects due
to possible nuclear accidents, occupational exposure nor due to radioactive waste disposal in underground facilities. Potential ionizing radiation from the soil, from
radon and from some construction materials is also not measured by this indicator.
8 / 12
Resource use
Indicator Unit A1 A2 A3 A4 C1 C2 C3 C4 D
PERE MJ 9,49E-01 2,79E-03 5,31E-02 2,56E-02 0,00E+00 3,93E-04 0,00E+00 2,14E-03 0,00E+00
PERM MJ 1,36E-01 0,00E+00 0,00E+00 0,00E+00 0,00E+00 0,00E+00 0,00E+00 0,00E+00 0,00E+00
PERT MJ 1,08E+00 2,79E-03 5,31E-02 2,56E-02 0,00E+00 3,93E-04 0,00E+00 2,14E-03 0,00E+00
PENRE MJ 2,25E+01 2,97E-01 1,19E+00 2,38E+00 0,00E+00 3,65E-02 0,00E+00 1,84E-01 0,00E+00
PENRM MJ 2,62E+00 0,00E+00 0,00E+00 0,00E+00 0,00E+00 0,00E+00 0,00E+00 0,00E+00 0,00E+00
PENRT MJ 2,51E+01 2,97E-01 1,19E+00 2,38E+00 0,00E+00 3,65E-02 0,00E+00 1,84E-01 0,00E+00
SM kg 5,15E-03 0,00E+00 3,01E-07 0,00E+00 0,00E+00 0,00E+00 0,00E+00 2,04E-05 0,00E+00
RSF MJ 1,93E-02 6,56E-05 5,70E-03 5,94E-04 0,00E+00 9,11E-06 0,00E+00 6,91E-05 0,00E+00
NRSF MJ 3,69E-03 5,24E-04 3,65E-04 3,58E-03 0,00E+00 5,49E-05 0,00E+00 2,69E-04 0,00E+00
FW m3 2,11E-02 2,92E-05 4,48E-04 2,90E-04 0,00E+00 4,45E-06 0,00E+00 9,17E-05 0,00E+00
PERE = Use of renewable primary energy excluding renewable primary energy resources used as raw materials; PERM = Use of renewable primary energy resources used
as raw materials; PERT = Total use of renewable primary energy resources; PENRE = Use of non renewable primary energy excluding non-renewable primary energy
resources used as raw materials; PENRM = Use of non renewable primary energy resources used as raw materials; PENRT = Total use of non renewable primary energy
resources; SM = Use of secondary materials; RSF = Use of renewable secondary fuels; NRSF = Use of non-renewable secondary fuels; FW = Net use of fresh water
"Reading example: 9,0 E-03 = 9,0*10-3 = 0,009"
*INA Indicator Not Assessed
9 / 12
End of life - Waste
Indicator Unit A1 A2 A3 A4 C1 C2 C3 C4 D
HWD kg 3,61E-03 1,93E-05 1,41E-04 1,82E-04 0,00E+00 2,79E-06 0,00E+00 1,14E-05 0,00E+00
NHWD kg 6,50E-01 1,72E-02 1,67E-02 2,05E-01 0,00E+00 3,14E-03 0,00E+00 5,15E-01 0,00E+00
RWD kg 3,34E-05 2,00E-06 1,40E-06 1,58E-05 0,00E+00 2,43E-07 0,00E+00 1,24E-06 0,00E+00
HWD = Hazardous waste disposed; NHWD = Non-hazardous waste disposed; RWD = Radioactive waste disposed
"Reading example: 9,0 E-03 = 9,0*10-3 = 0,009"
*INA Indicator Not Assessed
End of life - Output flow
Indicator Unit A1 A2 A3 A4 C1 C2 C3 C4 D
CRU kg 0,00E+00 0,00E+00 0,00E+00 0,00E+00 0,00E+00 0,00E+00 0,00E+00 0,00E+00 0,00E+00
MFR kg 3,74E-04 0,00E+00 5,13E-04 0,00E+00 0,00E+00 0,00E+00 0,00E+00 1,91E-05 0,00E+00
MER kg 1,88E-04 0,00E+00 2,97E-09 0,00E+00 0,00E+00 0,00E+00 0,00E+00 1,54E-07 0,00E+00
EEE MJ 8,60E-04 0,00E+00 1,12E-04 0,00E+00 0,00E+00 0,00E+00 0,00E+00 1,34E-06 0,00E+00
EET MJ 1,30E-02 0,00E+00 1,69E-03 0,00E+00 0,00E+00 0,00E+00 0,00E+00 2,02E-05 0,00E+00
CRU = Components for re-use; MFR = Materials for recycling; MER = Materials for energy recovery; EEE = Exported energy electrical; EET = Exported energy thermal
"Reading example: 9,0 E-03 = 9,0*10-3 = 0,009"
*INA Indicator Not Assessed
Biogenic Carbon Content
Indicator Unit At the factory gate
Biogenic carbon content in product kg C 0,00E+00
Biogenic carbon content in accompanying packaging kg C 4,99E-03
Note: 1 kg biogenic carbon is equivalent to 44/12 kg CO2
10 / 12
Additional requirements
Greenhouse gas emissions from the use of electricity in the manufacturing phase
National production mix from import, low voltage (production of transmission lines, in addition to direct emissions and losses in grid) of applied
electricity for the manufacturing process (A3).
Electricity mix Data source Amount Unit
Electricity, Indonesia (kWh) ecoinvent 3.6 1165,80 g CO2-eq/kWh
Dangerous substances
The product contains no substances on the REACH Candidate list at or above 100 ppm, 0,01 % by weight.
Indoor environment
The declared product is emission tested by RISE Research Institutes of Sweden/SP Technical Research Institute of Sweden or Eurofins in accordance
with California Department of Public Health (CDPH) Standard Method v1.2–2017.
Additional Environmental Information
Additional environmental impact indicators required in NPCR Part A for construction products
Indicator Unit A1 A2 A3 A4 C1 C2 C3 C4 D
GWPIOBC kg CO2 -eq 1,25E+00 2,06E-02 1,13E-01 1,55E-01 0,00E+00 2,37E-03 0,00E+00 9,92E-03 0,00E+00
GWP-IOBC: Global warming potential calculated according to the principle of instantaneous oxidation. In order to increase the transparency of biogenic carbon
contribution to climate impact, the indicator GWP-IOBC is required as it declares climate impacts calculated according to the principle of instantaneous oxidation.
GWP-IOBC is also referred to as GWP-GHG in context to Swedish public procurement legislation.
11 / 12
Bibliography
ISO 14025:2010 Environmental labels and declarations - Type III environmental declarations - Principles and procedures.
ISO 14044:2006 Environmental management - Life cycle assessment - Requirements and guidelines.
EN 15804:2012+A2:2019 Environmental product declaration - Core rules for the product category of construction products.
ecoinvent v3, Allocation, cut-off by classification, Swiss Centre of Life Cycle Inventories.
CEPE v3.0 Raw materials LCI database for the European coatings and printing ink industries, May 2016.
Iversen et al., (2021) eEPD v2021.09 Background information for EPD generator tool system verification, LCA.no Report number: 07.21
Vold et al (2017). EPD and LCA tool for Jotun - Technical description and background information, OR 01.17, Ostfold Research, Fredrikstad 2017.
Iversen, (2022) EPD generator for Jotun, Background information for re-verification of EPD generator application and LCA data, LCA.no report
number: 15.22
NPCR Part A: Construction products and services. Ver. 2.0. April 2021, EPD-Norge.
IBU PCR Part B: Requirements on the EPD for Coatings with organic binders. v1.7, April 2019.
BREEAM International (2021): BREEAM International New Construction Technical Manual - SD250. Ver. 6.0 (2021).
BREEAM International (2016): BREEAM International New Construction Technical Manual - SD233. Ver. 2.0 (2017).
CARB SCM (2020): California Air Resources Board (CARB) Suggested Control Measure for Architectural Coatings.
CDPH method 1.2 (2017): Standard method for the testing and evaluation of volatile organic chemical emissions from indoor sources. California
Department of Public Health.
LEED®v4.1 (2020): LEED® v4.1 for Building design and construction, U.S. Green Building Council®.
LEED®v4 (2013): LEED® v4 for Building design and construction, U.S. Green Building Council®.
REACH (2006): Regulation (EC) No 1907/2006 of the European Parliament and of the Council of 18 December 2006. REACH Authorization list –
Annex XIV, the Restriction list – Annex XVII and the SVHC candidate list.
Program operator and publisher Phone: +47 23 08 80 00
The Norwegian EPD Foundation e-mail: post@epd-norge.no
Post Box 5250 Majorstuen, 0303 Oslo, Norway web: www.epd-norge.no
Owner of the declaration: Phone: +47 33 45 70 00
Jotun A/S e-mail: cleo.otterbech@jotun.no
Hystadveien 167, 3209 Sandefjord web: www.jotun.no
Author of the Life Cycle Assessment Phone: +47 916 50 916
LCA.no AS e-mail: post@lca.no
Dokka 6B, 1671 web: www.lca.no
Developer of EPD generator Phone: +47 916 50 916
LCA.no AS e-mail: post@lca.no
Dokka 6B,1671 Kråkerøy web: www.lca.no
ECO Platform web: www.eco-platform.org
ECO Portal web: ECO Portal
12 / 12
