ver1 2015
ENVIRONMENTAL PRODUCT DECLARATION
in accordance with ISO 14025, ISO 21930 and EN 15804
Owner of the declaration: Elektroskandia Norge AS
Program operator: The Norwegian EPD Foundation
Publisher: The Norwegian EPD Foundation
Declaration number: NEPD-3149-1793-EN
Registration number: NEPD-3149-1793-EN
ECO Platform reference number: -
Issue date: 28.09.2021
Valid to: 28.09.2026
TSLI Pure 24kV AL 1x400/35mm² AFR
Elektroskandia Norge AS
www.epd-norge.no
NEPD-3149-1793-EN TSLI Pure 24kV AL 1x400/35mm² AFR
1 / 8
General information
Product: Owner of the declaration:
TSLI Pure 24kV AL 1x400/35mm² AFR Elektroskandia Norge AS
Contact person: Pål Kristiansen
Phone: +47 97 66 22 12
e-mail: pkr@elektroskandia.no
Program operator: Manufacturer:
Prysmian Group Norge AS
The Norwegian EPD Foundation
Kjerraten 16 3013 Drammen
Pb. 5250 Majorstuen, 0303 Oslo
Norway
Phone: +47 23 08 80 00
e-mail: post@epd-norge.no
Declaration number: Place of production:
Prysmian Group Sverige AB
NEPD-3149-1793-EN Vallgatan 5 571 41 Nässjö
Sweden
ECO Platform reference number: Management system:
ISO 14001, ISO 9001
This declaration is based on Product Category Rules: Organisation no:
977 454 700
CEN Standard EN 15804:2012+A1:2013 serves as core PCR
NPCR 027 Part B for Electrical cables and wires
Statement of liability: Issue date: 28.09.2021
The owner of the declaration shall be liable for the underlying information and
evidence. EPD Norway shall not be liable with respect to manufacturer Valid to: 28.09.2026
information, life cycle assessment data and evidences.
Declared unit: Year of study:
1 m TSLI Pure 24kV AL 1x400/35mm² AFR 2020
Declared unit with option: Comparability:
EPD of construction products may not be comparable if they not comply with EN
A1,A2,A3,A4,A5,C1,C2,C3,C4,D
15804 and seen in a building context.
Functional unit: Development and verification of EPD:
1 m of TSLI Pure 24 kV AL distribution power cable installed in a trench, The declaration has been developed and verified using EPD tool lca.tools
from cradle-to-grave. ver EPD2020.11, developed by LCA.no AS. The EPD tool is integrated into
the company's environmental management system, and has been
approved by EPD-Norway
General information on verification of EPD from EPD tools:
Independent verification of data, other environmental information and Developer of EPD:
the declaration according to ISO 14025:2010, § 8.1.3 and § 8.1.4. Individual
third party verification of each EPD is not required when the EPD tool is i) Ivan Ekerhovd, Prysmian Group Norge AS
integrated into the company's environmental management system, ii) the
procedures for use of the EPD tool are approved by EPDNorway, and iii) Reviewer of company-specific input data and EPD:
the proccess is reviewed annualy. See Appendix G of EPD-Norway's
General Programme Instructions for further information on EPD tools. Anders Nymark, Prysmian Group Norge AS
Verification of EPD tool: Approved:
Independent third party verification of the EPD tool, background data
Sign
and test-EPD in accordance with EPDNorway's procedures and guidelines
for verification and approval of EPD tools.
Fredrik Moltu Johnsen, Norsus AS
(no signature required) Håkon Hauan, CEO EPD-Norge
NEPD-3149-1793-EN TSLI Pure 24kV AL 1x400/35mm² AFR
2 / 8
Product
Product description: Technical data:
Halogen free and flame retardant. Smoke generation in the case of fire TSLI Pure 24kV AL 1x400/35mm² AFR
is small, low smoke density (makes evacuation easier) and is not Art.Nr: 20217597
harmful to electrical equipment. Distribution cable for indoor use in 3- Elnummer: 1060211
phase installation. Can be placed in pipes and in the ground. The cable
is axially and radially waterproof. Density: 2,3759 kg/m
Cenelec: N20XC7A5Z1-AR Produced according to
Building Installations, Power distribution HD 620 Part 10, Section K and M, HD604 (halogenfree sheath) Design
standard
Product specification
IEC 60332-3-24 (Cat. C) Flame retardant
Conductor material: Aluminium EN 60754-1 and EN 60754-2 Halogen free properties: EN 60754-1 (pH = 4,3,
Conductor surface: Bare Conductivity = 10µS), EN 60754-2 ( < 0,5% Halogen)
Longitudinal water blocking conductors: Yes Low smoke IEC 61034
Inner semi-conducting layer: Yes
Core insulation material: XLPE Market:
Outer semi-conducting layer: Yes
Scandinavia
Drain wire: Yes
Longitudinal water blocking cable: Yes Reference service life, product
Radial water blocking cable: Yes
The reference service life of the product is highly dependent on the
Screen construction: Aluminium tape and copper wire
conditions of use.
Screen: Yes
Screen material: Copper, Bare Reference service life, construcion
Concentric conductor: Copper Expected lifetime 50 years, provided proper installation, load and ambient
Material inner sheath: Other temperature.
Material outer sheath: Halogenfree polymer
Laminated sheath: Yes
Longitudinal water blocking screen: Yes
Cable shape: Round
Materials kg %
Aluminium 1,29 49,12
Copper 0,19 7,23
Other 0,65 24,96
Low Smoke Zero Halogen (LSZH) 0,49 18,70
Total: 2,62
Packaging kg
Packaging - Plastic strips 0,00
Total including packaging 2,62
LCA: Calculation rules
Declared unit: Allocation:
The allocation is made in accordance with the provisions of EN 15804.
1 m TSLI Pure 24kV AL 1x400/35mm² AFR
Incoming energy and water and waste production in-house is allocated
Cut-off criteria: equally among all products through mass allocation. Effects of primary
production of recycled materials is allocated to the main product in which
All major raw materials and all the essential energy is included. The
the material was used. The recycling process and transportation of the
production processes for raw materials and energy flows with very small
material is allocated to this analysis.
amounts (less than 1%) are not included. These cut-off criteria do not
apply for hazardous materials and substances.
Data quality:
Specific data for the product composition are provided by the manufacturer. They represent the production of the declared product and were collected for
EPD development in the year of study. Background data is based on registered EPDs according to EN 15804, Ostfold Research databases, ecoinvent and other
LCA databases. The data quality of the raw materials in A1 is presented in the table below.
Materials Source Data quality Year
Aluminium Supplier EPD 2017
Aluminium ecoinvent 3.6 Database 2019
Copper ecoinvent 3.6 Database 2019
Low Smoke Zero Halogen (LSZH) ecoinvent 3.6 Database 2019
Other ecoinvent 3.6 Database 2019
Packaging - Plastic strips ecoinvent 3.6 Database 2019
Aluminium NEPD-2261-1034-EN EPD 2020
NEPD-3149-1793-EN TSLI Pure 24kV AL 1x400/35mm² AFR
3 / 8
System boundary:
Additional technical information:
NEPD-3149-1793-EN TSLI Pure 24kV AL 1x400/35mm² AFR
4 / 8
LCA: Scenarios and additional technical information
The following information describe the scenarios in the different modules of the EPD.
In A4, a transport distance of 387 km from the Prysmian Group production site in Sweden to Elektroskandia’s warehouse in Langhus was included. A distance
of 300 km was also added as additional transport to market. Installation in trenches (A5) and removal (C1) is assumed to be done with other products such as
piping systems and should be assessed at a contruction works level. For B1-B7 the default environmental impact and resource indicators in the EPD are
assumed to be zero. Some other potential environmental impacts from the use phase might not be covered by the scope of an EPD. In C3 metals such as
copper and aluminium are sent to recycling and other materials such as plastic insulation is sent to municipal incineration. Net benefit of material recycling
and energy recovery is given in module D. Both aluminium and copper will replace a market average process for the metals in Europe.
Transport from production place to user (A4)
Capacity utilisation Fuel/Energy
Type Type of vehicle Distance km Unit Value (l/t)
(incl. return) % consumption
Truck 55,0 % Truck, lorry over 32 tonnes, EURO 5 687 0,022823 l/tkm 15,68
Railway l/tkm
Boat l/tkm
Other Transportation l/tkm
Assembly (A5) End of Life (C1, C3, C4)
. Unit Value . Unit Value
Auxiliary kg Hazardous waste disposed kg
Water consumption m3 Collected as mixed construction waste kg
Electricity consumption kWh Reuse kg
Other energy carriers MJ Recycling kg 1,3272
Material loss kg Energy recovery kg 1,1425
Output materials from waste treatment kg 0,0007 To landfill kg 0,2461
Dust in the air kg
VOC emissions kg
¨
Benefits and loads beyond the system boundaries (D)
. Unit Value
Substitution of primary Copper with net secondary copper (kg) kg 0,13
Substitution of primary Aluminium with net secondary aluminium (kg) kg 1,12
Substitution of electricity, in Norway (MJ) MJ 3,22
Substitution of thermal energy, district heating, in Norway (MJ) MJ 22,15
NEPD-3149-1793-EN TSLI Pure 24kV AL 1x400/35mm² AFR
5 / 8
LCA: Results
LCA results according to the indicators of EN 15804:2013+A1:2013 are presented in the following tables, for the declared unit defined on page 2 of the EPD
document. All potential environmental impacts might not be covered by the EN 15804 indicators. This concerns indicators such as noise, electromagnetic
radiation, electromagnetic fields and treatment brominated flame retardants.
System boundaries (X=included, MND=module not declared, MNR=module not relevant)
Construction Beyond the
Product stage installation User stage End of life stage . system
stage bondaries
A1 A2 A3 A4 A5 B1 B2 B3 B4 B5 B6 B7 C1 C2 C3 C4 . D
X X X X X X X X X . X
Environmental impact
Parameter Unit A1-A3 A4 A5 C1 C2 C3 C4 D
GWP kg CO 2 -eq 2,00E+01 1,42E-01 2,22E-03 0 0 3,03E+00 1,59E-02 -1,03E+01
ODP kg CFC11 -eq 1,23E-06 2,77E-08 4,00E-12 0 0 2,24E-08 1,12E-09 -8,76E-07
POCP kg C 2H 4-eq 9,66E-03 2,30E-05 4,91E-09 0 0 2,57E-05 1,78E-06 -7,49E-03
AP kg SO 2 -eq 2,02E-01 4,63E-04 2,42E-07 0 0 5,13E-04 3,76E-05 -1,18E-01
EP kg PO 3- -eq 1,76E-02 7,77E-05 7,57E-08 0 0 1,13E-04 6,26E-06 -7,24E-03
4
ADPM kg Sb -eq 1,14E-05 3,22E-07 5,70E-11 0 0 2,59E-07 1,39E-10 -3,93E-06
ADPE MJ 2,51E+02 2,23E+00 3,94E-04 0 0 9,20E-01 1,08E-01 -1,11E+02
GWP Global warming potential; ODP Depletion potential of the stratospheric ozone layer; POCP Formation potential of tropospheric photochemical oxidants;
AP Acidification potential of land and water; EP Eutrophication potential; ADPM Abiotic depletion potential for non fossil resources; ADPE Abiotic depletion
potential for fossil resources
"Reading example: 9,0 E-03 = 9,0*10-3 = 0,009"
*INA Indicator Not Assessed
waR slairetam tropsnarT gnirutcafunaM tropsnarT ylbmessA esU ecnanetniaM riapeR tnemecalpeR tnemhsibrufeR lanoitarepO ygrene esu lanoitarepO esu
retaw
-eD noitcurtsnoc noitilomed tropsnarT etsaW gnissecorp lasopsiD -yrevoceR-esueR -gnilcyceR laitnetop
NEPD-3149-1793-EN TSLI Pure 24kV AL 1x400/35mm² AFR
6 / 8
Resource use
Parameter Unit A1-A3 A4 A5 C1 C2 C3 C4 D
RPEE MJ 1,19E+02 4,04E-02 6,89E-06 0 0 1,16E-01 8,12E-03 -5,74E+01
RPEM MJ 0,00E+00 0,00E+00 0,00E+00 0 0 0,00E+00 0,00E+00 0,00E+00
TPE MJ 1,19E+02 4,04E-02 6,89E-06 0 0 1,16E-01 8,12E-03 -5,74E+01
NRPE MJ 2,52E+02 2,30E+00 3,15E-02 0 0 1,04E+00 1,19E-01 -1,39E+02
NRPM MJ 5,02E+01 0,00E+00 0,00E+00 0 0 0,00E+00 0,00E+00 0,00E+00
TRPE MJ 3,03E+02 2,30E+00 3,15E-02 0 0 1,04E+00 1,19E-01 -1,39E+02
SM kg 7,43E-02 0,00E+00 0,00E+00 0 0 0,00E+00 0,00E+00 0,00E+00
RSF MJ 9,33E-03 0,00E+00 0,00E+00 0 0 0,00E+00 0,00E+00 -6,35E-04
NRSF MJ 0,00E+00 0,00E+00 0,00E+00 0 0 0,00E+00 0,00E+00 0,00E+00
W m3 2,47E+01 5,43E-04 5,44E-07 0 0 3,14E-02 1,22E-04 -6,12E-02
RPEE Renewable primary energy resources used as energy carrier; RPEM Renewable primary energy resources used as raw materials; TPE Total use of renewable
primary energy resources; NRPE Non renewable primary energy resources used as energy carrier; NRPM Non renewable primary energy resources used as
materials; TRPE Total use of non renewable primary energy resources; SM Use of secondary materials; RSF Use of renewable secondary fuels; NRSF Use of non
renewable secondary fuels; W Use of net fresh water
"Reading example: 9,0 E-03 = 9,0*10-3 = 0,009"
*INA Indicator Not Assessed
End of life - Waste
Parameter Unit A1-A3 A4 A5 C1 C2 C3 C4 D
HW kg 4,95E-02 1,22E-06 2,36E-09 0 0 4,40E-06 1,29E-07 1,03E-02
NHW kg 2,33E+01 2,09E-01 4,71E-05 0 0 5,73E-02 3,39E-01 -8,46E+00
RW kg 1,24E-03 1,61E-05 1,58E-09 0 0 4,95E-06 7,17E-07 -5,87E-04
HW Hazardous waste disposed; NHW Non hazardous waste disposed; RW Radioactive waste disposed
"Reading example: 9,0 E-03 = 9,0*10-3 = 0,009"
*INA Indicator Not Assessed
End of life - Output flow
Parameter Unit A1-A3 A4 A5 C1 C2 C3 C4 D
CR kg 0,00E+00 0,00E+00 0,00E+00 0 0 0,00E+00 0,00E+00 0,00E+00
MR kg 2,09E-02 0,00E+00 0,00E+00 0 0 1,33E+00 0,00E+00 0,00E+00
MER kg 2,04E-03 0,00E+00 7,31E-04 0 0 1,14E+00 0,00E+00 0,00E+00
EEE MJ 1,33E-03 0,00E+00 1,56E-03 0 0 3,22E+00 0,00E+00 0,00E+00
ETE MJ 1,46E-02 0,00E+00 1,72E-02 0 0 2,21E+01 0,00E+00 0,00E+00
CR Components for reuse; MR Materials for recycling; MER Materials for energy recovery; EEE Exported electric energy; ETE Exported thermal energy
"Reading example: 9,0 E-03 = 9,0*10-3 = 0,009"
*INA Indicator Not Assessed
NEPD-3149-1793-EN TSLI Pure 24kV AL 1x400/35mm² AFR
7 / 8
Additional Norwegian requirements
Greenhouse gas emissions from the use of electricity in the manufacturing phase
National production mix from import, low voltage (production of transmission lines, in addition to direct emissions and losses in grid) of applied electricity for
the manufacturing process (A3).
Electricity mix Data source Amount Unit
El-mix, Sweden (kWh) ecoinvent 3.4 Alloc Rec 42,67 g CO2-ekv/kWh
Dangerous substances
The product contains no substances given by the REACH Candidate list or the Norwegian priority list.
Indoor environment
Not relevant, the cable is intended for outdoor use.
Bibliography
ISO 14025:2010 Environmental labels and declarations - Type III environmental declarations - Principles and procedures.
ISO 14044:2006 Environmental management - Life cycle assessment - Requirements and guidelines.
EN 15804:2012+A1:2013 Environmental product declaration - Core rules for the product category of construction products.
ISO 21930:2017 Sustainability in buildings and civil engineering works - Core rules for environmental product declarations of construction products.
ecoinvent v3, Allocation, cut-off by classification, Swiss Centre of Life Cycle Inventories.
Iversen et al., (2018) eEPD v3- Background information for EPD generator system. LCA.no report 04.18. Iversen et al., (2020) EPD generator for Elektroskandia and Prysmian Group
- Background information and LCA data, LCA.no report 01.20
NPCR Part A: Construction products and services. Ver. 1.04.2017 EPD-Norge. NPCR 27 Part B for electrical cables and wires or NPCR 28 Part B for cable pipes Ver. 1.02.2020 EPD-
Norge.
Program operator and publisher Phone: +47 23 08 80 00
The Norwegian EPD Foundation e-mail: post@epd-norge.no
Post Box 5250 Majorstuen, 0303 Oslo,Norway web: www.epd-norge.no
Owner of the declaration Phone: +47 97 66 22 12
Elektroskandia Norge AS e-mail: pkr@elektroskandia.no
Postboks 143 1403 Langhus web: elektroskandia.no
Author of the Life Cycle Assessment Phone: +47 916 50 916
LCA.no AS e-mail: post@lca.no
Dokka 1C 1671 Kråkerøy web: www.lca.no
Developer of EPD generator Phone: +47 916 50 916
LCA.no AS e-mail: post@lca.no
Dokka 1C,1671 Kråkerøy web: www.lca.no
NEPD-3149-1793-EN TSLI Pure 24kV AL 1x400/35mm² AFR
8 / 8
