Environmental product declaration
in accordance with ISO 14025 and EN 15804+A2
PE 100-RC Extruded Sheets GPA SE
Owner of the declaration: Program operator:
GPA Flowsystem AS The Norwegian EPD Foundation
Product: Declaration number:
PE 100-RC Extruded Sheets GPA SE
NEPD-8839-8495
Declared unit:
1 kg Registration number:
This declaration is based on Product Category Rules: NEPD-8839-8495
CEN Standard EN 15804:2012+A2:2019 serves as core
Issue date: 27.01.2025
PCR
NPCR 031:2023 Part B for sea-based aquaculture Valid to: 27.01.2030
infrastructure and components
The Norwegian EPD Foundation EPD software:
LCAno EPD generator ID: 766313
1 / 11
General information
Product Owner of the declaration:
PE 100-RC Extruded Sheets GPA SE GPA Flowsystem AS
Contact person: Aleksander Haugen Knutsen
Phone: +47 48133609
e-mail: info@gpa.no
Program operator: Manufacturer:
The Norwegian EPD Foundation AGRU Kunststofftechnik GmbH
Post Box 5250 Majorstuen, 0303 Oslo, Norway
Phone: +47 977 22 020
web: www.epd-norge.no
Declaration number: Place of production:
AGRU Kunststofftechnik GmbH
NEPD-8839-8495
Ing.-Pesendorfer-Straße 31
4540 Bad Hall, Austria
This declaration is based on Product Category Rules: Management system:
CEN Standard EN 15804:2012+A2:2019 serves as core PCR ISO 9001 and ISO 14001
NPCR 031:2023 Part B for sea-based aquaculture infrastructure and
components
Statement of liability: Organisation no:
The owner of the declaration shall be liable for the underlying 936 875 025
information and evidence. EPD Norway shall not be liable with respect
to manufacturer information, life cycle assessment data and
evidences.​
Declared unit: Issue date:
1 kg PE 100-RC Extruded Sheets GPA SE 27.01.2025
Declared unit with option: Valid to:
A1,A2,A3,A4,C1,C2,C3,C4,D 27.01.2030
Year of study:
2022
Functional unit: Comparability:
EPD of construction products may not be comparable if they not
comply with EN 15804 and seen in a building context.
General information on verification of EPD from EPD tools: Development and verification of EPD:
Independent verification of data, other environmental information The declaration is created using EPD tool lca.tools ver EPD2022.03,
and the declaration according to ISO 14025:2010, § 8.1.3 and § 8.1.4. developed by LCA.no. The EPD tool is integrated in the company's
Verification of each EPD is made according to EPD-Norway’s management system, and has been approved by EPD Norway.
guidelines for verification and approval requiring that tools are i)
integrated into the company's environmental management system, ii) Developer of EPD: Måns Sjögren
the procedures for use of the EPD tool are approved by EPD-Norway,
Reviewer of company-specific input data and EPD:​ Tobias Antonsen
and iii) the process is reviewed annually by an independent third
party verifier. See Appendix G of EPD-Norway's General Programme
Instructions for further information on EPD tools
Verification of EPD tool: Approved:
Independent third party verification of the EPD tool, background data
and test-EPD in accordance with EPDNorway's procedures and
guidelines for verification and approval of EPD tools. Approval
number: NEPDT65.
Third party verifier:
Elisabet Amat, GREENIZE projects
(no signature required)
2 / 11
Product
Product description:
This EPD covers polyethylene (PE) sheets with a thickness from 1mm to 40mm for use in a wide range of applications, including tank containers,
vats, prefabrication of parts, flotation devices for floating docks.
Product specification
EPD covers the following product ranges: PEP21, PEP31, PEP42, PEP62
Materials kg %
Plastic - Polyethylene (HDPE) 1,00 100,00
Total 1,00 100,00
Technical data:
EPD covers polyethylene (PE) sheets from thickness 1mm to 40mm, in the sizes 2000x1000mm, 3000x1500mm, 4000x2000mm and
6000x2000mm.
PE material with density 960kg/m3
Market:
Sweden
Reference service life, product
100 years
Reference service life, building or construction works
100 years
LCA: Calculation rules
Declared unit:
1 kg PE 100-RC Extruded Sheets GPA SE
Cut-off criteria:
All major raw materials and all the essential energy is included. The production processes for raw materials and energy flows with very small
amounts (less than 1%) are not included. These cut-off criteria do not​ apply for hazardous materials and substances.
Allocation:
The allocation is made in accordance with the provisions of EN 15804. Incoming energy and water and waste production in-house is allocated
equally among all products through mass allocation. Effects of primary production of recycled materials is allocated to the main product in which
the material was used. The recycling process and transportation of the material is allocated to this analysis.
Data quality:
Specific data for the product composition are provided by the manufacturer. The data represent the production of the declared product and were
collected for EPD development in the year of study. Background data is based on EPDs according to EN 15804 and different LCA databases. The
data quality of the raw materials in A1 is presented in the table below.
Materials Source Data quality Year
Plastic - Polyethylene (HDPE) ecoinvent 3.6 Database 2019
3 / 11
System boundaries (X=included, MND=module not declared, MNR=module not relevant)
Construction Beyond the system
Product stage Use stage End of life stage
installation stage boundaries
A1 A2 A3 A4 A5 B1 B2 B3 B4 B5 B6 B7 C1 C2 C3 C4 D
X X X X MND MND MND MND MND MND MND MND X X X X X
System boundary:
Additional technical information:
Packaging material is not included in this EPD, but can be provided for project specific EPD on request.
waR slairetam tropsnarT gnirutcafunaM tropsnarT ylbmessA e​sU ecnanetniaM riapeR tnemecalpeR tnemhsibrufeR lanoitarepO ygrene esu lanoitarepO esu retaw -eD noitcurtsnoc noitilomed tropsnarT etsaW gnissecorp lasopsiD -yrevoceR-esueR laitnetop-gnilcyceR
4 / 11
LCA: Scenarios and additional technical information
The following information describe the scenarios in the different modules of the EPD.
A4: The sheets are transported 1250km from Bad Hall, Austria to Hjärnarp, Sweden before delivery to customer which is set to 300km. The
distance of 300km is given in newer PCRs as a default value for Swedish domestic transport.
A5: Has not been included due to there being several ways of installation. Project specific EPDs available on request.
C1-C4: Has not been included as it is assumed that the sheets are left as is after end of life.
Capacity utilisation Value
Transport from production place to user (A4) Distance (km) Fuel/Energy Consumption Unit
(incl. return) % (Liter/tonne)
Truck, 16-32 tonnes, EURO 6 (km) - Europe 36,7 % 1250 0,043 l/tkm 53,75
Truck, 16-32 tonnes, EURO 6 (km) - Europe 36,7 % 300 0,043 l/tkm 12,90
5 / 11
LCA: Results
The LCA results are presented below for the declared unit defined on page 2 of the EPD document.
Environmental impact
Indicator Unit A1 A2 A3 A4 C1 C2 C3 C4 D
GWP-total kg CO2 -eq 2,01E+00 2,99E-03 2,42E-01 2,53E-01 0 0 0 0 0
GWP-fossil kg CO2 -eq 2,00E+00 2,97E-03 2,41E-01 2,53E-01 0 0 0 0 0
GWP-biogenic kg CO2 -eq 1,04E-02 1,32E-05 3,09E-04 1,05E-04 0 0 0 0 0
GWP-luluc kg CO2 -eq 6,13E-04 5,66E-06 3,87E-05 9,01E-05 0 0 0 0 0
ODP kg CFC11 -eq 5,10E-08 3,00E-10 5,25E-08 5,74E-08 0 0 0 0 0
AP mol H+ -eq 7,20E-03 1,82E-05 5,66E-04 7,28E-04 0 0 0 0 0
EP-FreshWater kg P -eq 3,40E-05 2,17E-07 3,02E-06 2,02E-06 0 0 0 0 0
EP-Marine kg N -eq 1,23E-03 3,76E-06 1,27E-04 1,44E-04 0 0 0 0 0
EP-Terrestial mol N -eq 1,37E-02 4,31E-05 1,43E-03 1,61E-03 0 0 0 0 0
POCP kg NMVOC -eq 6,69E-03 1,22E-05 4,76E-04 6,17E-04 0 0 0 0 0
ADP-minerals&metals1 kg Sb-eq 1,79E-05 2,88E-08 1,48E-06 6,99E-06 0 0 0 0 0
ADP-fossil1 MJ 7,08E+01 4,87E-02 3,58E+00 3,83E+00 0 0 0 0 0
WDP1 m3 7,48E+01 4,71E-01 5,38E+02 3,70E+00 0 0 0 0 0
GWP-total = Global Warming Potential total; GWP-fossil = Global Warming Potential fossil fuels; GWP-biogenic = Global Warming Potential biogenic; GWP-luluc =
Global Warming Potential land use and land use change; ODP = Depletion potential of the stratospheric ozone layer; AP = Acidification potential, Accumulated
Exceedance; EP-freshwater = Eutrophication potential, fraction of nutrients reaching freshwater end compartment: EP-marine = Eutrophication potential, fraction of
nutrients reaching marine end compartment; EP-terrestrial = Eutrophication potential, Accumulated Exceedance; POCP = Formation potential of tropospheric ozone;
ADP-minerals&metals = Abiotic depletion potential for non-fossil resources; ADP-fossil = Abiotic depletion for fossil resources potential; WDP = Water (user)
deprivation potential, deprivation-weighted water consumption
"Reading example: 9,0 E-03 = 9,0*10-3 = 0,009"
*INA Indicator Not Assessed
1. The results of this environmental impact indicator shall be used with care as the uncertainties on these results are high or as there is limited experienced with the
indicator
Remarks to environmental impacts
6 / 11
Additional environmental impact indicators
Indicator Unit A1 A2 A3 A4 C1 C2 C3 C4 D
PM Disease incidence 5,96E-08 1,50E-10 3,92E-09 1,55E-08 0 0 0 0 0
IRP2 kgBq U235 -eq 4,72E-02 3,34E-04 2,73E-03 1,67E-02 0 0 0 0 0
ETP-fw1 CTUe 1,10E+01 5,36E-02 1,59E+00 2,84E+00 0 0 0 0 0
HTP-c1 CTUh 5,41E-10 0,00E+00 7,70E-11 0,00E+00 0 0 0 0 0
HTP-nc1 CTUh 1,23E-08 7,50E-11 1,78E-09 3,10E-09 0 0 0 0 0
SQP1 dimensionless 2,24E+00 3,62E-02 2,54E-01 2,68E+00 0 0 0 0 0
PM = Particulate Matter emissions; IRP = Ionizing radiation – human health; ETP-fw = Eco toxicity – freshwater; HTP-c = Human toxicity – cancer effects; HTP-nc =
Human toxicity – non cancer effects; SQP = Potential Soil Quality Index (dimensionless)
"Reading example: 9,0 E-03 = 9,0*10-3 = 0,009"
*INA Indicator Not Assessed
1. The results of this environmental impact indicator shall be used with care as the uncertainties on these results are high or as there is limited experienced with the
indicator
2. This impact category deals mainly with the eventual impact of low dose ionizing radiation on human health of the nuclear fuel cycle. It does not consider effects due
to possible nuclear accidents, occupational exposure nor due to radioactive waste disposal in underground facilities. Potential ionizing radiation from the soil, from
radon and from some construction materials is also not measured by this indicator.
7 / 11
Resource use
Indicator Unit A1 A2 A3 A4 C1 C2 C3 C4 D
PERE MJ 1,19E+00 6,68E-03 1,60E+00 5,48E-02 0 0 0 0 0
PERM MJ 0,00E+00 0,00E+00 0,00E+00 0,00E+00 0 0 0 0 0
PERT MJ 1,19E+00 6,68E-03 1,60E+00 5,48E-02 0 0 0 0 0
PENRE MJ 3,14E+01 4,88E-02 3,59E+00 3,83E+00 0 0 0 0 0
PENRM MJ 4,25E+01 0,00E+00 0,00E+00 0,00E+00 0 0 0 0 0
PENRT MJ 7,39E+01 4,88E-02 3,59E+00 3,83E+00 0 0 0 0 0
SM kg 0,00E+00 0,00E+00 0,00E+00 0,00E+00 0 0 0 0 0
RSF MJ 7,07E-02 4,85E-04 7,23E-03 1,96E-03 0 0 0 0 0
NRSF MJ 8,98E-03 1,85E-04 1,95E-03 7,01E-03 0 0 0 0 0
FW m3 2,42E-02 3,53E-05 5,09E-03 4,09E-04 0 0 0 0 0
PERE = Use of renewable primary energy excluding renewable primary energy resources used as raw materials; PERM = Use of renewable primary energy resources used
as raw materials; PERT = Total use of renewable primary energy resources; PENRE = Use of non renewable primary energy excluding non-renewable primary energy
resources used as raw materials; PENRM = Use of non renewable primary energy resources used as raw materials; PENRT = Total use of non renewable primary energy
resources; SM = Use of secondary materials; RSF = Use of renewable secondary fuels; NRSF = Use of non-renewable secondary fuels; FW = Net use of fresh water
"Reading example: 9,0 E-03 = 9,0*10-3 = 0,009"
*INA Indicator Not Assessed
8 / 11
End of life - Waste
Indicator Unit A1 A2 A3 A4 C1 C2 C3 C4 D
HWD kg 1,36E-03 8,25E-06 5,78E-03 1,97E-04 0 0 0 0 0
NHWD kg 6,36E-02 7,32E-04 1,50E-02 1,86E-01 0 0 0 0 0
RWD kg 4,21E-05 2,95E-07 3,73E-06 2,61E-05 0 0 0 0 0
HWD = Hazardous waste disposed; NHWD = Non-hazardous waste disposed; RWD = Radioactive waste disposed
"Reading example: 9,0 E-03 = 9,0*10-3 = 0,009"
*INA Indicator Not Assessed
End of life - Output flow
Indicator Unit A1 A2 A3 A4 C1 C2 C3 C4 D
CRU kg 0,00E+00 0,00E+00 0,00E+00 0,00E+00 0 0 0 0 0
MFR kg 0,00E+00 0,00E+00 2,05E-03 0,00E+00 0 0 0 0 0
MER kg 0,00E+00 0,00E+00 2,37E-03 0,00E+00 0 0 0 0 0
EEE MJ 0,00E+00 0,00E+00 2,90E-06 0,00E+00 0 0 0 0 0
EET MJ 0,00E+00 0,00E+00 4,39E-05 0,00E+00 0 0 0 0 0
CRU = Components for re-use; MFR = Materials for recycling; MER = Materials for energy recovery; EEE = Exported energy electrical; EET = Exported energy thermal
"Reading example: 9,0 E-03 = 9,0*10-3 = 0,009"
*INA Indicator Not Assessed
Biogenic Carbon Content
Indicator Unit At the factory gate
Biogenic carbon content in product kg C 0,00E+00
Biogenic carbon content in accompanying packaging kg C 0,00E+00
Note: 1 kg biogenic carbon is equivalent to 44/12 kg CO2
9 / 11
Additional requirements
Greenhouse gas emissions from the use of electricity in the manufacturing phase
National production mix from import, low voltage (production of transmission lines, in addition to direct emissions and losses in grid) of applied
electricity for the manufacturing process (A3).
Electricity mix Source Amount Unit
Electricity, guarantee of origin, low voltage, for AGRU factory In Austria (kWh) Modified ecoinvent 3.6 301,58 g CO2-eq/kWh
Dangerous substances
The product contains no substances given by the REACH Candidate list.
Indoor environment
Additional Environmental Information
Additional environmental impact indicators required in NPCR Part A for construction products
Indicator Unit A1 A2 A3 A4 C1 C2 C3 C4 D
GWPIOBC kg CO2 -eq 1,90E+00 2,99E-03 2,40E-01 2,53E-01 0 0 0 0 0
GWP-IOBC: Global warming potential calculated according to the principle of instantaneous oxidation. In order to increase the transparency of biogenic carbon​
contribution to climate impact, the indicator GWP-IOBC is required as it declares climate impacts calculated according to the principle of instantaneous oxidation.​
GWP-IOBC is also referred to as GWP-GHG in context to Swedish public procurement legislation.
10 / 11
Bibliography
ISO 14025:2010. Environmental labels and declarations - Type III environmental declarations - Principles and procedures. International
Organization for Standardization.
ISO 14044:2006. Environmental management - Life cycle assessment - Requirements and guidelines. International Organization for
Standardization.
EN 15804:2012+A2:2019. Environmental product declaration - Core rules for the product category of construction products. European
Committee for Standardization.
ISO 21930:2017. Sustainability in buildings and civil engineering works - Core rules for environmental product declarations of construction
products. International Organization for Standardization.
Ecoinvent v3, 2019. Allocation, cut-off by classification. Swiss Centre of Life Cycle Inventories.
Iversen et al., (2021). eEPD v2021.09, background information for EPD generator tool system verification, LCA.no. Report number: 07.21. System
verification report.
Gaspard Philis (2023). EPD generator for NPCR 031 part B for aquaculture infrastructure and components, Background information for EPD
generator application and LCA data, LCA.no report number: 03.23. PCR verification report.
EPD Norway (2022). NPCR Part A: Construction products and services. The Norwegian EPD foundation. Version 2.0 published 24.03.2021.
EPD Norway (2023). NPCR 031 Part B for aquaculture infrastructure and components. The Norwegian EPD foundation. Version 1.0 published
26.04.2023.
ISO 14632 - Extruded sheets of polyethylene (PE-HD)
Program operator and publisher Phone: +47 977 22 020
The Norwegian EPD Foundation e-mail: post@epd-norge.no
Post Box 5250 Majorstuen, 0303 Oslo, Norway web: www.epd-norge.no
Owner of the declaration: Phone:
+47 48133609
GPA Flowsystem AS e-mail:
info@gpa.no
Regnbueveien 9, 1405 Langhus, Norway web:
Author of the Life Cycle Assessment Phone: +47 916 50 916
LCA.no AS e-mail: post@lca.no
Dokka 6A, 1671 Kråkerøy, Norway web: www.lca.no
Developer of EPD generator Phone: +47 916 50 916
LCA.no AS e-mail: post@lca.no
Dokka 6A, 1671 Kråkerøy, Norway web: www.lca.no
ECO Platform web: www.eco-platform.org
ECO Portal web: ECO Portal
11 / 11
