Environmental Product
Declaration
In accordance with ISO 14025 and EN 15804 +A1
Kvillsfors inward and outward opening doors – K1, D1, P1, G1
(with aluminium cladding)
Owner of the declaration:
NorDan AS Product name:
Program holder and publisher: Kvillsfors inward and
outward opening doors – K1,
D1, P1, G1 (with aluminium
The Norwegian EPD foundation
Declaration number: cladding)
N ReE gP iD s- t3 ra4 t4 i9 o- n2 0 N5 u9 m-E bN
e r: Manufacturer:
NorDan AS
NEPD-3449-2059-EN
Issue date:
Valid to:
02.05.2022
The Norwegian 02.05.2027
EPD Foundation
General information
Product: Owner of the declaration:
Kvillsfors inward and outward opening doors – K1, D1, P1, G1 (with NorDan AS
aluminium cladding) Kontaktperson: Fredrik Jonsson
Tlf: +46 (0) 10-130 01 78
e-post: fredrik.jonsson@nordan.se
Program holder: Manufacturer:
The Norwegian EPD Foundation
Post Box 5250 Majorstuen, 0303 Oslo NorDan AB
Tlf: +47 977 22 020 Grebbestadsvägen 8 457 91 Tanumshede
e-mail: post@epd-norge.no
Phone: +46 (0)10 - 130 00 00
Declaration number: Place of production:
NEPD-3449-2059-EN Kvillsfors, Sweden
ECO Platform registration number: Management system:
-
This declaration is based on Product Category Rules: NorDan AB. Works with EN ISO 9001:2015, ISO 14001:2015
CEN Standard EN 15804 serves as core PCR NPCR014:2019
version 3.0 Part B for Windows and doors Org. no.:
NO 979 776 233 MVA
Declaration of responsibility: Issue date:
The owner of the declaration shall be responsible for the 02.05.2022
underlying information and evidence. EPD Norway shall not be
responsible with regard to manufacturer information, life cycle data
and evidence.
Valid to:
02.05.2027
Declared unit: Year of study:
2021
Declared unit with option: Comparability:
EPD of construction products may not be comparable if they are
not comply with NS-EN 15804 and seen in a building context.
Functional unit:
1 door set measuring 1.23 m x 2.18 m (reference door based on EN
14351-1) with an essential parameter U-value = 1,0 - 1,2 and with an The EPD has been worked out by:
expected service life of 60 years. Conversion factor is 98.51 [Kg/FU]. Roja Modaresi
Norsk Treteknisk Institutt
Verification:
Independent verification of the declaration and data,
according to ISO14025:2010
internal external
Approved
Third party verifier:
Gaylord K. Booto PhD., Senior Research Scientist, NORSUS AS
(Independent verifier approved by EPD Norway)
NEPD-3449-2059-EN Kvillsfors inward and outward opening doors – K1, D1, P1, G1 (with aluminium cladding)
2/9
Product
Product description: Technical data:
Balcony door for use in exterior walls of domestic and commercial Balcony door. Triple glazed or double glazed with secondary
buildings. sash, 115mm frame with aluminium clad. Uwin 1,0 - 1,2 W/m2K.
Manufactured in accordance with ISO 9001:2008 and
ISO14001:2015. Certified: Bluesky, SP Sitac “P”,
Product specification:
25% of aluminium and 7% of glass is produced from recycled The total product weight is 98.51 kg. The packaging has an
material. average weight of 5.6 kg.
Product group K1, D1, P1, G1 is covered in this EPD. The highest
amount for constituent material has been used.
Materialer kg %
Pine timber 22.87 23.22 Market:
Glue for timber 0.13 0.13
Glass 59.97 60.88 Europe, but scenarios beyond cradle to gate are based
Spacer 0.29 0.30 on the situation in the Norwegian market.
Butyl 0.02 0.02
Triple glazed unit
Sealant 0.29 0.30
Absorbent 0.13 0.13
Argon 0.05 0.05
Paint 1.16 1.18 Reference service life:
Aluminium 7.98 8.10 The reference service life is 60 years for aluminium cladding
Plastic 0.02 0.02 timber frame
Gasket 1.41 1.43
Metal 3.85 3.90
Glue 0.04 0.04
Glass list 0.31 0.31
Total weight of the product 98.51 100
Wood packaging 5.31
Steel packaging 0.05
Plastic packaging 0.12
cardboard packaging 0,4
Total weight with packaging 103.99
LCA: Calculation rules
Functional unit: System boundary:
1 door set measuring 1.23 m x 2.18 m (reference door based on EN All modules are included. Below is a technical flowchart for the
14351-1) with an essential parameter U-value = 1,0 - 1,2 and with an production line at Nordan. Modul D is calculated with energy
expected service life of 60 years. Conversion factor is 98.51 [Kg/FU]. substitution and explained in the scenarios.
NEPD-3449-2059-EN Kvillsfors inward and outward opening doors – K1, D1, P1, G1 (with aluminium cladding)
3/9
Data quality Cut-off criteria:
Data is representative of year 2020 and was collected in 2021-2022. All raw materails and energy use is included. Where data was
Data is taken from processes from Ecoinvent 3.1-3.7. Some processes available for infrastructure from Ecoinvent, it is included.
are based on Ecoinvent v3.1 (2014) and v3.2 (2015), but all upstream Example: ‘Metal working factory'. In the production process, raw
processes are v3.4 (2017)-3.5 (2018). Remaining data is based on materials and energy of low amounts are not included (<1%).
Ecoinvent v3.7 (2020). "Allocation cut-off by classification" adjusted to These cut-off rules do not apply to dangerous substances.
improve representativeness.
Allocation: Calculations of biogenic carbon:
Allocation is done in accordance with the provisions of EN 15804. Sequestration and release of biogenic carbon is included
Allocation of energy, water and waste from production is calculated by a according to EN 16485:2014. This is based on the modularity
physical allocation factor based on the manufacturer input. For waste principle in EN 15804:2012 that specifies that the emissions
produced at the manufacturing, the burdens for reuse, recycling and shall be accounted in the module that they occur. The amount of
recovery is allocated by using this allocation factor. carbon dioxide sequestrated is calulated in accordance to EN
16449:2014. Timber comes from sustainable forestry and has
FSC certified traceability.
LCA: Scenarios and additional technical information
The following information describe the scenarios in the different modules of the EPD
The transportation from production to construction site is based on a scenario where the product is transported on a large lorry from Kvillsfors,
Sweden to Oslo, Norway (500 km) and then to a warehouse which is assumed to be in a 250 km radius from Oslo. Transport from warehouse
to a construction site is assumed to be 50 km on a medium truck.
Transport from production place to assembly/user (A4)
Type Capacity utilisation Type of vehicle Distance km Fuel/Energy Fuel/Energy
(incl. return) % consumption pr tkm consumption pr km
Truck 53 EURO5, >32 tonn 750 0.023 l/tkm 0.31 l/km
Truck 26 EURO5, 16-32 tonn 50 0.045 l/tkm 0.25 l/km
Installation (A5)
Unit Value According to the report from EPD-Norge ‘Harmonising the documentation
Auxiliary kg 0 of scenarios beyond cradle to gate, EN 15804’ there is no loss on site
Water consumption m3 0 during construction activities. The window products in this EPD are
Electricity consumption MJ 0 painted and surface treated in the production and not at the building site.
Other energy carriers MJ 0 Therefore, there is only 2 items left in this module. 1) Waste treatment of
Material loss kg 0 packaging which is considered in the EPD calculations. 1) Energy use
Output materials from waste treatment kg 5.48 during installation. This can be varied depending on the floor, type of
Dust in the air kg 0 building and several other unknown parameters, and therefore ignored in
the calculation.
Maintenance (B2)/Repair (B3)
The maintenance scenario included cleaning, painting and change of
Unit Value (alu cladding) IGU. Cleaning is performed three times per year. It is calculated with 1,5
dl of detergent and 3 litres of water each year. Windows with aluminium
Detergents kg 9
cladding are assumed to be painted 3 times during its lifetime from
Water consumption l 180
inside. It is assumed that 5 gr of lubricating oil is used every year for
Lubricating oil kg 0.30 fittings and moving parts. The glazing unit is changed once during the
Paint kg 0.55 lifetime for the windows with aluminium cladding. No repair is assumed
Transport tkm 2.95 during the product lifetime.
Glazing unit kg 60.75
Synthetic rubber kg 1.41
Transport (IGU) tkm 18.23
NEPD-3449-2059-EN Kvillsfors inward and outward opening doors – K1, D1, P1, G1 (with aluminium cladding)
4/9
Replacement (B4)/Refurbishment (B5)
*Number or RSL (Reference Service Life). The window has RSL of 60
Unit Value years. Therefore, it is assumed to replace the insulated glass unit after 30
Replacement cycle* yr 60 years (See Module B4). There is no need for refurbishment during the
Electricity consumption kWh 0 product lifetime.
Replacement of worn parts 0 0
(C1) As there are no data for de-construction, it is assumed no activites in C1 in this study. The windows are assumed to be treated as mixed
waste and sent to incineration. The combustible materials are then energy recovered, while glass is assumed to end up in the bottom ash and
then landfilled. The metals are usually sorted out of the bottom ash and then recycled, but there is no data of the share which are recycled and
therefore standard values from Ecoinvent is utilized.
The transport of window as waste is calculated based on a scenario with 50 km distance.
Transport to waste processing (C2)
Type Capacity utilisation Type of vehicle Distance km Fuel/Energy Fuel/Energy
(incl. return) % consumption pr tkm consumption pr km
Truck 44 Unspecified 50 0.03l/tkm 0.28 l/km
Windows are assumed to be sorted as mixed construction waste and treated with incineration with energy recovery. However, the
manufacturer has documented the recycling potentials for its product in the Construction Product Declaration eBVD
Kvillsfors Utåtgående Kopplad Dörr - K1, ID: C-SE556294452901-126 URL: https://www.ebvd.org/BMI/Document/Export/6677/0/Pdf Kvillsfors
Utåtgående Dörr - D1, ID: C-SE556294452901-138 URL: https://www.ebvd.org/BMI/Document/Export/7403/0/Pdf Kvillsfors inåtgående Dörr -
P1, ID: C-SE556294452901-125 URL: https://www.ebvd.org/BMI/Document/Export/6672/0/Pdf Kvillsfors inåtgående Dörr - G1, ID: C-
SE556294452901-137 URL: https://www.ebvd.org/BMI/Document/Export/7353/0/Pdf
In the documentation, Chapter 10, the specific material recovery, and energy recovery potential is reported for the product.
End of Life (C1, C3, C4)
Unit Value
Hazardous waste disposed kg 0
Collected as mixed construction waste kg 98.51
Reuse kg 0
Recycling kg 4.70
Energy recovery kg 93.81
To landfill kg 0.00
The benefits beyond life cycle has been modelled based on the output flows from module C3. This includes energy from incineration and scrap
metal recovered from the ashes. The amount recovered metal is assumed to avoid production of primary metals in accordance to 6.4.3.3 in EN
15804. The exported energy is substituting Norwegian district heating mix and electricity mix. Inventory processes causing substitution of avoided
virgin raw materials has be constructed for each material.
Benefits and loads beyond the system boundaries (D)
Value (alu
Unit cladding)
Substitution of electricity MJ 41.8
Substitution of thermal energy MJ 383.2
Substitution of raw materials kg 4.8
NEPD-3449-2059-EN Kvillsfors inward and outward opening doors – K1, D1, P1, G1 (with aluminium cladding)
5/9
LCA: Results
Global warming potential in A1-A3 includes sequestration of CO2 as carbon in the wood. This amount is accounted as an emission in module
C3. Additionally, it is included sequestration in the wood packaging. This is accounted as an emission in module A5. The flow of biogenic
carbon for the system is presented in page 9.
System boundaries (X = included)
A2 A5 B4
X X X X X X X X X
Environmental impact With alu clad
Parameter Unit A4 A5 B1 B2
GWP kg CO -ekv 1.74E+02 6.43E+00 8.42E+00 0.00E+00 1.23E+02 0.00E+00 0.00E+00
2
kg CFC11-ekv 1.78E-05 1.25E-06 0.00E+00 0.00E+00 1.00E-05 1.00E+00 0.00E+00
POCP kg CH -ekv 1.34E-01 7.54E-04 0.00E+00 0.00E+00 0.00E+00
2 4
AP kg SO -ekv 1.45E+00 1.63E-02 0.00E+00 0.00E+00 8.44E-01 3.00E+00 0.00E+00 0.00E+00
2
EP kg PO3--ekv 1.46E-01 2.23E-03 0.00E+00 0.00E+00 8.32E-02 4.00E+00 0.00E+00 0.00E+00
4
ADPM kg Sb-ekv 5.37E-03 1.68E-05 0.00E+00 0.00E+00 5.25E-04 5.00E+00 0.00E+00 0.00E+00
ADPE MJ 2.38E+03 1.03E+02 0.00E+00 0.00E+00 1.49E+03 6.00E+00 0.00E+00 0.00E+00
Parameter Unit B6 B7 C1 C2 C3 C4 D
GWP kg CO -ekv 0.00E+00 0.00E+00 0.00E+00 6.19E-01 4.85E+01 7.83E-01 -6.41E+01
2
ODP kg CFC11-ekv 0.00E+00 0.00E+00 0.00E+00 1.13E-07 6.42E-08 2.08E-07 -1.96E-06
POCP kg CH -ekv 0.00E+00 0.00E+00 0.00E+00 7.81E-05 3.84E-04 1.80E-04 -2.32E-02
2 4
AP kg SO -ekv 0.00E+00 0.00E+00 0.00E+00 1.96E-03 5.84E-03 4.38E-03 -3.53E-01
2
EP kg PO3--ekv 0.00E+00 0.00E+00 0.00E+00 3.23E-04 1.76E-03 8.09E-04 -3.28E-02
4
ADPM kg Sb-ekv 0.00E+00 0.00E+00 0.00E+00 2.09E-06 1.57E-06 1.56E-06 -8.90E-05
ADPE MJ 0.00E+00 0.00E+00 0.00E+00 9.35E+00 1.28E+02 1.87E+01 -6.03E+02
GWP Global warming potential; ODP Depletion potential of the stratospheric ozone layer; POCP Formation potential of tropospheric photochemical
oxidants; AP Acidification potential of land and water; EP Eutrophication potential; ADPM Abiotic depletion potential for non fossil resources; ADPE Abiotic
depletion potential for fossil resources.
noitallatsni
noitcurtsnoC
egats esU
tnemhsibrufeR
B6 D
ODP
3.64E-02 2.00E+00 0.00E+00
gnissecorp
etsaW
lasopsiD
Beyond the
system
boundaries
C4
X X
riapeR
End of Life stage
B3 C1
X X
tropsnarT tropsnarT
esu
ygrene
lanoitarepO
Construction
Product stage and installation
stage
B1 B2 C2
X X X X
esu
retaw
lanoitarepO
noitcurtsnoc-eD
noitilomed tropsnarT
C3
-yrevoceR-esueR laitnetop
gnilcyceR
Use stage
A1
slairetam
waR
A3 A4
gnirutcafunaM ecnanetniaM
B5
tnemecalpeR
B7
A1-A3 B3 B4 B5
0.00E+00
0.00E+00
NEPD-3449-2059-EN Kvillsfors inward and outward opening doors – K1, D1, P1, G1 (with aluminium cladding)
6/9
Resource use with alu clad
Parameter Unit A1-A3 A4 A5 B1 B2 B3 B4 B5
RPEE MJ 1.0E+03 1.3E+00 0.0E+00 0.0E+00 9.6E+01 0.0E+00 0.0E+00 0.0E+00
RPEM MJ 4.7E+02 0.0E+00 0.0E+00 0.0E+00 0.0E+00 0.0E+00 0.0E+00 0.0E+00
TPE MJ 1.5E+03 1.3E+00 0.0E+00 0.0E+00 9.6E+01 0.0E+00 0.0E+00 0.0E+00
NRPE MJ 2.9E+03 1.0E+02 0.0E+00 0.0E+00 1.6E+03 0.0E+00 0.0E+00 0.0E+00
NRPM MJ 9.4E+01 0.0E+00 0.0E+00 0.0E+00 -4.6E+01 0.0E+00 0.0E+00 0.0E+00
TRPE MJ 3.0E+03 1.0E+02 0.0E+00 0.0E+00 1.5E+03 0.0E+00 0.0E+00 0.0E+00
SM kg 2.2E+00 0.0E+00 0.0E+00 0.0E+00 0.0E+00 0.0E+00 0.0E+00 0.0E+00
RSF MJ 2.4E-01 0.0E+00 0.0E+00 0.0E+00 1.4E-01 0.0E+00 0.0E+00 0.0E+00
NRSF MJ 1.5E-01 0.0E+00 0.0E+00 0.0E+00 8.6E-02 0.0E+00 0.0E+00 0.0E+00
W m3 3.5E+00 1.1E-02 0.0E+00 0.0E+00 1.4E+00 0.0E+00 0.0E+00 0.0E+00
Resource use with alu clad
Parameter Unit B6 B7 C1 C2 C3 C4 D
RPEE MJ 0.0E+00 0.0E+00 0.0E+00 1.3E-01 3.8E+02 2.8E-01 -2.6E+02
RPEM MJ 0.0E+00 0.0E+00 0.0E+00 0.0E+00 -3.8E+02 0.0E+00 0.0E+00
TPE MJ 0.0E+00 0.0E+00 0.0E+00 1.3E-01 9.3E-01 2.8E-01 -2.6E+02
NRPE MJ 0.0E+00 0.0E+00 0.0E+00 9.6E+00 1.3E+02 1.9E+01 -6.1E+02
NRPM MJ 0.0E+00 0.0E+00 0.0E+00 0.0E+00 -1.2E+02 0.0E+00 0.0E+00
TRPE MJ 0.0E+00 0.0E+00 0.0E+00 9.6E+00 6.6E+00 1.9E+01 -6.1E+02
SM kg 0.0E+00 0.0E+00 0.0E+00 0.0E+00 0.0E+00 0.0E+00 0.0E+00
RSF MJ 0.0E+00 0.0E+00 0.0E+00 0.0E+00 6.2E-01 0.0E+00 -1.6E+02
NRSF MJ 0.0E+00 0.0E+00 0.0E+00 0.0E+00 4.1E-01 0.0E+00 -1.0E+02
W m3 0.0E+00 0.0E+00 0.0E+00 1.0E-03 2.0E-02 1.7E-02 -9.1E-01
RPEE Renewable primary energy resources used as energy carrier; RPEM Renewable primary energy resources used as raw materials; TPE Total use of
renewable primary energy resources; NRPE Non renewable primary energy resources used as energy carrier; NRPM Non renewable primary energy
resources used as materials; TRPE Total use of non renewable primary energy resources; SM Use of secondary materials; RSF Use of renewable
secondary fuels; NRSF Use of non renewable secondary fuels; W Use of net fresh water.
End of life-Waste with alu clad
Parameter Unit A1-A3 A4 A5 B1 B2 B3 B4 B5
HW kg 2.94E+00 5.52E-03 0.00E+00 0.00E+00 6.75E+01 0.00E+00 0.00E+00 0.00E+00
NHW kg 6.25E+01 8.71E+00 0.00E+00 0.00E+00 1.99E+01 0.00E+00 0.00E+00 0.00E+00
RW kg 1.47E-02 7.18E-04 0.00E+00 0.00E+00 4.79E-03 0.00E+00 0.00E+00 0.00E+00
End of life-Waste with alu clad
Parameter Unit B6 B7 C1 C2 C3 C4 D
HW kg 0.00E+00 0.00E+00 0.00E+00 4.98E-04 8.32E-03 7.45E+01 -5.58E-01
NHW kg 0.00E+00 0.00E+00 0.00E+00 6.14E-01 2.10E-01 6.15E-01 -1.16E+01
RW kg 0.00E+00 0.00E+00 0.00E+00 6.53E-05 2.27E-05 1.19E-04 -8.05E-04
HW Hazardous waste disposed; NHW Non hazardous waste disposed; RW Radioactive waste disposed
End of life- Output flow with alu clad
Parameter Unit A1-A3 A4 A5 B1 B2 B3 B4 B5
CR kg 0.00E+00 0.00E+00 0.00E+00 0.00E+00 0.00E+00 0.00E+00 0.00E+00 0.00E+00
MR kg 2.19E+00 0.00E+00 5.70E-01 0.00E+00 3.25E-01 0.00E+00 0.00E+00 0.00E+00
MER kg 0.00E+00 0.00E+00 5.31E+00 0.00E+00 0.00E+00 0.00E+00 0.00E+00 0.00E+00
EEE MJ 1.55E+01 0.00E+00 0.00E+00 0.00E+00 8.84E+00 0.00E+00 0.00E+00 0.00E+00
ETE MJ 1.62E+02 0.00E+00 0.00E+00 0.00E+00 6.11E+01 0.00E+00 0.00E+00 0.00E+00
End of life- Output flow with alu clad
Parameter Unit B6 B7 C1 C2 C3 C4 D
CR kg 0.00E+00 0.00E+00 0.00E+00 0.00E+00 0.00E+00 0.00E+00 0.00E+00
MR kg 0.00E+00 0.00E+00 0.00E+00 0.00E+00 4.70E+00 0.00E+00 -4.79E+00
MER kg 0.00E+00 0.00E+00 0.00E+00 0.00E+00 0.00E+00 0.00E+00 0.00E+00
EEE MJ 0.00E+00 0.00E+00 0.00E+00 0.00E+00 4.11E+01 0.00E+00 -4.18E+01
ETE MJ 0.00E+00 0.00E+00 0.00E+00 0.00E+00 2.85E+02 0.00E+00 -3.83E+02
CR Components for reuse; MR Materials for recycling; MER Materials for energy recovery; EEE Exported electric energy; ETE Exported thermal energy
Reading example: 9,0 E-03 = 9,0*10-3 = 0,009
NEPD-3449-2059-EN Kvillsfors inward and outward opening doors – K1, D1, P1, G1 (with aluminium cladding)
7/9
Norwegian additional requirements
Greenhouse gas emissions from the use of electricity in the production phase
National (Sweden) market with low-voltage, including imports, direct emissions, infrastructure and transmission losses, has been used for
electricity in the production process (A3). The manufacturer is documented the use of electricity from hydropower with guarantees of origin,
which has 6 fold less GWP effect. However, the final result has only be improved by 0.6% in A1-A3 production. Therfore, the national
electricity mix is considerd.
Data source Quantity Unit
Ecoinvent v3.7 (september 2020) 41 gram CO 2-ekv./kWh
Hazardous substances
The product contains no substances from REACH Candidate List or the Norwegian Priority List
The product contains substances below 0.1% by weight on the REACH Candidate List
The product contains substances from REACH Candidate List or the Norwegian Priority List, see table under Specific
Norwegian requirements.
The product does not contain any substances on the REACH Candidate List or the Norwegian Priority List. The product can be
characterized as hazardous waste (according to the Waste Shift, Appendix III), see table under Specific Norwegian requirements.
Transport
Transport from production site to construction site according to scenario in A4: 750+50 km
Indoor air quality
The product has not been tested for emissions to indoor environments.
Carbon footprint
To increase the transparency of the climate impacts, the GWP indicator has been divided into sub-indicators:
GWP-IOBC Climate impacts calculated according to instant oxidation principle
GWP-BCIP Climate impacts calculated from the net impacts of sequestration and emission of biogenic carbon
Climate impact with alu clad
Parameter Unit A1-A3 A4 A5 B1 B2 B3 B4 B5
GWP-IOBC kg CO -ekv 2.19E+02 6.43E+00 0.00E+00 0.00E+00 1.23E+02 0.00E+00 0.00E+00 0.00E+00
2
GWP-BCIP kg CO -ekv -4.45E+01 0.00E+00 8.42E+00 0.00E+00 0.00E+00 0.00E+00 0.00E+00 0.00E+00
2
GWP kg CO -ekv 1.75E+02 6.43E+00 8.42E+00 0.00E+00 1.23E+02 0.00E+00 0.00E+00 0.00E+00
2
Climate impact with alu clad
Parameter Unit B6 B7 C1 C2 C3 C4 D
GWP-IOBC kg CO -ekv 0.00E+00 0.00E+00 0.00E+00 6.19E-01 1.24E+01 7.83E-01 -6.41E+01
2
GWP-BCIP kg CO -ekv 0.00E+00 0.00E+00 0.00E+00 0.00E+00 3.61E+01 0.00E+00 0.00E+00
2
GWP kg CO -ekv 0.00E+00 0.00E+00 0.00E+00 6.19E-01 4.85E+01 7.83E-01 -6.41E+01
2
Additional information
For the products with different sizes from the declared unit, the environmental impacts must be converted by using a conversion factor. The
Norwegian EPD Foundation has published instructions on how to interpret EPDs for windows on its website (www.epd-norge.no) where
different calculation methods have been stated. (Document: Bruksanvisninger i hvordan tolke EPD'er – Vinduer)
NEPD-3449-2059-EN Kvillsfors inward and outward opening doors – K1, D1, P1, G1 (with aluminium cladding)
8/9
Bibliografi
NS-EN ISO 14025:2010 Miljømerker og deklarasjoner - Miljødeklarasjoner type III - Prinsipper og prosedyrer.
NS-EN ISO 14044:2006 Miljøstyring - Livsløpsvurderinger - Krav og retningslinjer
NS-EN 15804:2012+A1:2013 Bærekraftig byggverk - Miljødeklarasjoner - Grunnleggende produktkategoriregler for byggevarer
ISO 21930:2007 Sustainability in building construction - Environmental declaration of building products
Modaresi, R. 2020 LCA-report for Nordan LCA-report nr. 325039-1 from Norwegian Institute of Wood Technology,
Oslo, Norway.
NPCR014 (04/2019) Product category rules for windows and doors, rev3, April 2019
NS-EN 16485:2014 Tømmer og skurlast - Miljødeklarasjoner - Produktkategoriregler for tre og trebaserte produkter til
bruk i byggverk
NS-EN 16449:2014 Tre og trebaserte produkter - Beregning av biogent karboninnhold i tre og omdanning til
karbondioksid
Ecoinvent v3.0-3.7 Ecoinvent database version 3.0-3.7 Centre for Life Cycle Inventories.
Statistisk sentralbyrå Tabell 04727: Fjernvarmebalansen, 2015
Statistisk sentralbyrå Tabell 09469: Nettoproduksjon av fjernvarme, 2015
NEPD-307-179-NO EPD for skurlast av gran eller furu. Treindustrien
Bruksanvisninger i hvordan tolke EPD'er – Vinduer. https://www.epd-norge.no [in Norwegian]
Publisher Tlf: +47 23 08 80 00
The Norwegian EPD Foundation
Postboks 5250 Majorstuen, 0303 Oslo e-post: post@epd-norge.no
Norway web www.epd-norge.no
Owner of the declaration Tlf: +47 51 40 40 00
NorDan AS
Stasjonsveien 46, N-4460 Moi e-post: firmapost@nordan.no
Norway
web www.nordan.no
Author of the Life Cycle Assessment Tlf: +47 98 85 33 33
Roja Modaresi
Norsk Treteknisk Instiutt e-post: firmapost@treteknisk.no
Postboks 113 Blindern, 0314 Oslo, Norway web www.treteknisk.no
NEPD-3449-2059-EN Kvillsfors inward and outward opening doors – K1, D1, P1, G1 (with aluminium cladding)
9/9
EPD for the best
environmental
decision
www.epd-norge.no
The Norwegian EPD foundation
EPD for the best environmental decision
12
