Environmental product declaration
In accordance with 14025 and EN15804+A2
PE100 RC Pressure Sewage pipes in coil SDR 17
Owner of the declaration: Program operator:
Pipelife Sverige AB The Norwegian EPD Foundation
Product: Declaration number:
PE100 RC Pressure Sewage pipes in coil SDR 17
Registration number:
Declared unit:
1 kg Issue date:
22.05.2023
This declaration is based on Product Category Rules:
CEN Standard EN 15804:2012+A2:2019 serves as core Valid to:
PCR 22.05.2028
The Norwegian EPD Foundation
NPCR Part A: Construction products and services. Ver.
EPD Software:
1.0. March 2021
LCA.no EPD generator ID: 62879
1 / 11
General information
Product Owner of the declaration:
PE100 RC Pressure Sewage pipes in coil SDR 17 Pipelife Sverige AB
Contact person:
Phone: +46 513 22114
e-mail: yvette.lennartsson@pipelife.com
Program operator: Manufacturer:
Post Box 5250 Majorstuen, 0303 Oslo, Norway Pipelife Sverige AB
The Norwegian EPD Foundation
Phone: +47 23 08 80 00
web: post@epd-norge.no
Declaration number: Place of production:
Pipelife Sverige AB
Box 50
SE-524 02 Ljung , Sweden
This declaration is based on Product Category Rules: Management system:
CEN Standard EN 15804:2012+A2:2019 serves as core PCR EN ISO 9001:2015 and EN ISO 14001:2015
NPCR Part A: Construction products and services. Ver. 1.0. March
2021
Statement of liability: Organisation no:
The owner of the declaration shall be liable for the underlying SE556087042901
information and evidence. EPD Norway shall not be liable with respect
to manufacturer information, life cycle assessment data and
evidences.​
Declared unit: Issue date:
1 kg PE100 RC Pressure Sewage pipes in coil SDR 17 22.05.2023
Declared unit (cradle to gate) with option: Valid to:
A1-A3,A4,C1,C2,C3,C4,D 22.05.2028
Year of study:
2022
Functional unit: Comparability:
EPD of construction products may not be comparable if they not
comply with EN 15804 and seen in a building context.
General information on verification of EPD from EPD tools: Development and verification of EPD:
Independent verification of data, other environmental information The declaration is created using EPD tool lca.tools ver EPD2022.03,
and the declaration according to ISO 14025:2010, § 8.1.3 and § 8.1.4. developed by LCA.no. The EPD tool is integrated in the company's
Individual​ third party verification of each EPD is not required when management system, and has been approved by EPD Norway.
the EPD tool is i) integrated into the company's environmental
management system, ii) the procedures for use of the EPD tool are Developer of EPD: Yvette Lennartsson
approved by EPDNorway, and iii)​ the proccess is reviewed annualy.
Reviewer of company-specific input data and EPD: Mattias Petersson
See Appendix G of EPD-Norway's General Programme Instructions
for further information on EPD tools.
Verification of EPD tool: Approved:
Independent third party verification of the EPD tool, background data
and test-EPD in accordance with EPDNorway's procedures and
guidelines for verification and approval of EPD tools.
Third party verifier:
Michael M. Jenssen, Asplan Viak AS Håkon Hauan, CEO EPD-Norge
(no signature required)
2 / 11
Product
Product description:
Conformity mark covered by certificate; Nordic Poly Mark
Product specification
70021071, 70021070, 70021024, 70020951, 70020949, 70021037, 70021030, 70021026, 70023226, 70023227, 70023228, 70023229,
70023230, 70023231, 70023232, 70023237, 70023238, 70023239, 70023240, 70023241, 70023242, 70023243, 70023244, 70023245,
70023246
Product related data to be found at Pipelife Sverige AB product catalogue https://catalog.pipelife.com/se
Materials kg %
Polyethylene (HDPE) 1,00 100,00
Total 1,00
Technical data:
PE material with density 960 kg/m3.
Produced according SS EN 12201
Raw material certified by PAS 1075
Market:
Europe, with scenario made for the Swedish market.
Reference service life, product
Lifetime on product calculated more than 100 years.
Reference service life, building
LCA: Calculation rules
Declared unit:
1 kg PE100 RC Pressure Sewage pipes in coil SDR 17
Cut-off criteria:
All major raw materials and all the essential energy is included. The production processes for raw materials and energy flows with very small
amounts (less than 1%) are not included. These cut-off criteria do not​ apply for hazardous materials and substances.
Allocation:
The allocation is made in accordance with the provisions of EN 15804. Incoming energy and water and waste production in-house is allocated
equally among all products through mass allocation. Effects of primary production of recycled materials is allocated to the main product in which
the material was used. The recycling process and transportation of the material is allocated to this analysis.
Data quality:
Specific data for the product composition are provided by the manufacturer. They represent the production of the declared product and were
collected for EPD development in the year of study. Background data is based on registered EPDs according to EN 15804, Ostfold Research
databases, ecoinvent and other LCA databases. The data quality of the raw materials in A1 is presented in the table below.​
Materials Source Data quality Year
Polyethylene (HDPE) ecoinvent 3.6 Database 2019
3 / 11
System boundaries (X=included, MND=module not declared, MNR=module not relevant)
Construction Beyond the system
Product stage Use stage End of life stage
installation stage boundaries
A1 A2 A3 A4 A5 B1 B2 B3 B4 B5 B6 B7 C1 C2 C3 C4 D
X X X X MND MND MND MND MND MND MND MND X X X X X
System boundary:
Additional technical information:
Conformity mark covered by certificate; Nordic Poly Mark
waR slairetam tropsnarT gnirutcafunaM tropsnarT ylbmessA e​sU ecnanetniaM riapeR tnemecalpeR tnemhsibrufeR lanoitarepO ygrene esu lanoitarepO esu retaw -eD noitcurtsnoc noitilomed tropsnarT etsaW gnissecorp lasopsiD -yrevoceR-esueR laitnetop-gnilcyceR
4 / 11
LCA: Scenarios and additional technical information
The following information describe the scenarios in the different modules of the EPD.
A5 - "Assemly", refer to NPCR 019 Part B Piping systems A2.
C1 - C4 "End of life stage", we assume that the pipes will remain within the ground, therefore no data input.
D - "Beyond the system boundaries", we assume that the pipes will remain in the ground, therefore no data input.
Capacity utilisation Value
Transport from production place to user (A4) Distance (km) Fuel/Energy Consumption Unit
(incl. return) % (Liter/tonne)
Truck, 16-32 tonnes, EURO 6 (km) 36,7 % 100 0,043 l/tkm 4,30
5 / 11
LCA: Results
The LCA results are presented below for the declared unit defined on page 2 of the EPD document.
Environmental impact
Indicator Unit A1-A3 A4 C1 C2 C3 C4 D
GWP-total kg CO2 -eq 2,23E+00 1,63E-02 0 0 0 0 0
GWP-fossil kg CO2 -eq 2,22E+00 1,63E-02 0 0 0 0 0
GWP-biogenic kg CO2 -eq 1,17E-02 6,76E-06 0 0 0 0 0
GWP-luluc kg CO2 -eq 3,27E-03 5,81E-06 0 0 0 0 0
ODP kg CFC11 -eq 1,06E-07 3,70E-09 0 0 0 0 0
AP mol H+ -eq 8,27E-03 4,69E-05 0 0 0 0 0
EP-FreshWater kg P -eq 3,93E-05 1,31E-07 0 0 0 0 0
EP-Marine kg N -eq 1,52E-03 9,29E-06 0 0 0 0 0
EP-Terrestial mol N -eq 1,71E-02 1,04E-04 0 0 0 0 0
POCP kg NMVOC -eq 7,64E-03 3,98E-05 0 0 0 0 0
ADP-minerals&metals1 kg Sb -eq 2,37E-05 4,51E-07 0 0 0 0 0
ADP-fossil1 MJ 7,80E+01 2,47E-01 0 0 0 0 0
WDP1 m3 5,55E+02 2,39E-01 0 0 0 0 0
GWP total = Global Warming Potential total; GWP fossil = Global Warming Potential fossil fuels ; GWP biogenic = Global Warming Potential biogenic; GWP luluc =
Global W Potential land use change; ODP = Ozone Depletion; AP = Acidification; EP freshwater = Eutrophication aquatic freshwater; EP = marine Eutrophication aquatic
marine; EP = terrestrial Eutrophication terrestrial ;POCP = Photochemical zone formation; ADPE = Abiotic Depletion Potential minerals and metals; ADPF = Abiotic
Depletion Potential fossil fuels;
"Reading example: 9,0 E-03 = 9,0*10-3 = 0,009"
*INA Indicator Not Assessed
1. The results of this environmental impact indicator shall be used with care as the uncertainties on these results are high or as there is limited experienced with the
indicator
Remarks to environmental impacts
6 / 11
Additional environmental impact indicators
Indicator Unit A1-A3 A4 C1 C2 C3 C4 D
PM Disease incidence 7,60E-08 1,00E-09 0 0 0 0 0
IRP2 kgBq U235 -eq 2,19E-01 1,08E-03 0 0 0 0 0
ETP-fw1 CTUe 1,55E+01 1,83E-01 0 0 0 0 0
HTP-c1 CTUh 6,68E-10 0,00E+00 0 0 0 0 0
HTP-nc1 CTUh 1,69E-08 2,00E-10 0 0 0 0 0
SQP1 dimensionless 5,82E+00 1,73E-01 0 0 0 0 0
PM = Particulate Matter emissions; IRP = Ionizing radiation – human health; ETP-fw = Eco toxicity – freshwater; HTP-c = Human toxicity – cancer effects; HTP-nc =
Human toxicity – non cancer effects; SQP = Soil Quality (dimensionless)
"Reading example: 9,0 E-03 = 9,0*10-3 = 0,009"
*INA Indicator Not Assessed
1. The results of this environmental impact indicator shall be used with care as the uncertainties on these results are high or as there is limited experienced with the
indicator
2. This impact category deals mainly with the eventual impact of low dose ionizing radiation on human health of the nuclear fuel cycle. It does not consider effects due
to possible nuclear accidents, occupational exposure nor due to radioactive waste disposal in underground facilities. Potential ionizing radiation from the soil, from
radon and from some construction materials is also not measured by this indicator.
7 / 11
Resource use
Indicator Unit A1-A3 A4 C1 C2 C3 C4 D
PERE MJ 3,50E+00 3,54E-03 0 0 0 0 0
PERM MJ 0,00E+00 0,00E+00 0 0 0 0 0
PERT MJ 3,50E+00 3,54E-03 0 0 0 0 0
PENRE MJ 3,87E+01 2,47E-01 0 0 0 0 0
PENRM MJ 4,25E+01 0,00E+00 0 0 0 0 0
PENRT MJ 8,12E+01 2,47E-01 0 0 0 0 0
SM kg 5,71E-03 0,00E+00 0 0 0 0 0
RSF MJ 8,38E-02 1,26E-04 0 0 0 0 0
NRSF MJ 4,39E-02 4,52E-04 0 0 0 0 0
FW m3 8,36E-02 2,64E-05 0 0 0 0 0
PERE Use of renewable primary energy excluding renewable primary energy resources used as raw materials; PERM Use of renewable primary energy resources used as
raw materials; PERT Total use of renewable primary energy resources; PENRE Use of non renewable primary energy excluding non-renewable primary energy resources
used as raw materials; PENRM Use of non renewable primary energy resources used as raw materials; PENRT Total use of non renewable primary energy resources; SM
Use of secondary materials; RSF Use of renewable secondary fuels; NRSF Use of non renewable secondary fuels; FW Use of net fresh water
"Reading example: 9,0 E-03 = 9,0*10-3 = 0,009"
*INA Indicator Not Assessed
8 / 11
End of life - Waste
Indicator Unit A1-A3 A4 C1 C2 C3 C4 D
HWD kg 4,54E-03 1,27E-05 0 0 0 0 0
NHWD kg 1,81E-01 1,20E-02 0 0 0 0 0
RWD kg 1,29E-04 1,68E-06 0 0 0 0 0
HWD = Hazardous waste disposed; NHWD = Non-hazardous waste disposed; RWD = Radioactive waste disposed;
"Reading example: 9,0 E-03 = 9,0*10-3 = 0,009"
*INA Indicator Not Assessed
End of life - Output flow
Indicator Unit A1-A3 A4 C1 C2 C3 C4 D
CRU kg 0,00E+00 0,00E+00 0 0 0 0 0
MFR kg 7,35E-04 0,00E+00 0 0 0 0 0
MER kg 1,60E-02 0,00E+00 0 0 0 0 0
EEE MJ 1,12E-02 0,00E+00 0 0 0 0 0
EET MJ 1,70E-01 0,00E+00 0 0 0 0 0
CRU = Components for re-use; MFR = Materials for recycling; MER = Materials for energy recovery; EEE = Exported energy electrical; EET = Exported energy Thermal;
"Reading example: 9,0 E-03 = 9,0*10-3 = 0,009"
*INA Indicator Not Assessed
Biogenic Carbon Content
Indicator Unit At the factory gate
Biogenic carbon content in product kg C 0,00E+00
Biogenic carbon content in accompanying packaging kg C 0,00E+00
Note: 1 kg biogenic carbon is equivalent to 44/12 kg CO2
9 / 11
Additional Norwegian requirements
Greenhouse gas emissions from the use of electricity in the manufacturing phase
National production mix from import, low voltage (production of transmission lines, in addition to direct emissions and losses in grid) of applied
electricity for the manufacturing process (A3).
Electricity mix Data source Amount Unit
Electricity, Sweden (kWh) ecoinvent 3.6 54,94 g CO2-eq/kWh
Dangerous substances
No substances given by the REACH Candidate list or the Norwegian priority list are intentionally added to the product.
Indoor environment
Additional Environmental Information
Environmental impact indicators EN 15804+A2 and NPCR Part A v2.0
Indicator Unit A1-A3 A4 C1 C2 C3 C4 D
GWP kg CO2 -eq 2,10E+00 1,62E-02 0 0 0 0 0
ODP kg CFC11 -eq 1,15E-07 3,00E-09 0 0 0 0 0
POCP kg C2H4 -eq 6,38E-04 1,97E-06 0 0 0 0 0
AP kg SO2 -eq 6,42E-03 3,23E-05 0 0 0 0 0
EP kg PO43- -eq 5,99E-04 3,43E-06 0 0 0 0 0
ADPM kg Sb -eq 2,32E-05 4,51E-07 0 0 0 0 0
ADPE MJ 7,33E+01 2,42E-01 0 0 0 0 0
GWPIOBC kg CO2 -eq 2,09E+00 1,63E-02 0 0 0 0 0
GWP Global warming potential; ODP Depletion potential of the stratospheric ozone layer; POCP Formation potential of tropospheric photochemical oxidants; AP
Acidification potential of land and water; EP Eutrophication potential; ADPM Abiotic depletion potential for non fossil resources; ADPE Abiotic depletion​ potential for
fossil resources; GWP-IOBC/GHG Global warming potential calculated according to the principle of instantanious oxidation (except emissions and uptake of biogenic
carbon)
10 / 11
Bibliography
ISO 14025:2010 Environmental labels and declarations - Type III environmental declarations - Principles and procedures.
ISO 14044:2006 Environmental management - Life cycle assessment - Requirements and guidelines.
EN 15804:2012+A2:2019 Environmental product declaration - Core rules for the product category of construction products.
ISO 21930:2017 Sustainability in buildings and civil engineering works - Core rules for environmental product declarations of construction
products.
ecoinvent v3, Allocation, cut-off by classification, Swiss Centre of Life Cycle Inventories.
Iversen et al., (2021) eEPD v2021.09 Background information for EPD generator tool system verification, LCA.no rapportnummer: : 07.21.
Vold, et al., (2019) EPD generator for Pipelife - Background information for customer application and LCA data. report number 08.19
NPCR Part A: Construction products and services. Ver. 2.0. March 2021, EPD-Norge.
Program operator and publisher Phone: +47 23 08 80 00
The Norwegian EPD Foundation e-mail: post@epd-norge.no
Post Box 5250 Majorstuen, 0303 Oslo, Norway web: www.epd-norge.no
Owner of the declaration: Phone: +46 513 22114
Pipelife Sverige AB e-mail: yvette.lennartsson@pipelife.com
Box 50 , SE-524 02 Ljung web:
Author of the Life Cycle Assessment Phone: +47 916 50 916
LCA.no AS e-mail: post@lca.no
Dokka 6B, 1671 web: www.lca.no
Developer of EPD generator Phone: +47 916 50 916
LCA.no AS e-mail: post@lca.no
Dokka 6B,1671 Kråkerøy web: www.lca.no
ECO Platform web: www.eco-platform.org
ECO Portal web: ECO Portal
11 / 11
