Environmental product declaration
in accordance with ISO 14025 and EN 15804+A2
Enclosure ENC 160 1530 60
Owner of the declaration: Program operator:
AKVA group ASA The Norwegian EPD Foundation
Product: Declaration number:
Enclosure ENC 160 1530 60 57288
Declared unit: Registration number:
1 pcs 57288
This declaration is based on Product Category Rules: Issue date:
CEN Standard EN 15804:2012+A2:2019 serves as core 14.07.2023
PCR
The Norwegian EPD Foundation NPCR 031:2023 Part B for sea-based aquaculture Valid to:
infrastructure and components 14.07.2026
EPD Software:
LCA.no EPD generator ID: 57288
1 / 12
General information
Product Owner of the declaration:
Enclosure ENC 160 1530 60 AKVA group ASA
Contact person: Trude Olafsen
Phone: +47 91557400
e-mail: tolafsen@akvagroup.com
Program operator: Manufacturer:
Post Box 5250 Majorstuen, 0303 Oslo, Norway AKVA group ASA
The Norwegian EPD Foundation
Phone: +47 23 08 80 00
web: post@epd-norge.no
Declaration number: Place of production:
57288 AKVA group ASA
Plogfabrikkvegen 11
4353 Klepp Stasjon, Norway
This declaration is based on Product Category Rules: Management system:
CEN Standard EN 15804:2012+A2:2019 serves as core PCR
NPCR 031:2023 Part B for sea-based aquaculture infrastructure and
components
Statement of liability: Organisation no:
The owner of the declaration shall be liable for the underlying 931 693 670
information and evidence. EPD Norway shall not be liable with respect
to manufacturer information, life cycle assessment data and
evidences.​
Declared unit: Issue date:
1 pcs Enclosure ENC 160 1530 60 14.07.2023
Declared unit with option: Valid to:
A1,A2,A3,A4,C1,C2,C3,C4,D 14.07.2026
Year of study:
2021
Functional unit: Comparability:
1 piece of impregnated enclosure manufactured and delivered at the EPD of construction products may not be comparable if they not
sea-farm, including waste treatment at end-of-life. comply with EN 15804 and seen in a building context.
General information on verification of EPD from EPD tools: Development and verification of EPD:
Independent verification of data, other environmental information The declaration is created using EPD tool lca.tools ver EPD2022.03,
and the declaration according to ISO 14025:2010, § 8.1.3 and § 8.1.4. developed by LCA.no. The EPD tool is integrated in the company's
Verification of each EPD is made according to EPD-Norway’s management system, and has been approved by EPD Norway.
guidelines for verification and approval requiring that tools are i)
integrated into the company's environmental management system, ii) Developer of EPD: Karen Kvalheim
the procedures for use of the EPD tool are approved by EPD-Norway,
Reviewer of company-specific input data and EPD:​ Elisabet Amat -
and iii) the process is reviewed annually by an independent third
GREENIZE projects
party verifier. See Appendix G of EPD-Norway's General Programme
Instructions for further information on EPD tools
Verification of EPD tool: Approved:
Independent third party verification of the EPD tool, background data
and test-EPD in accordance with EPDNorway's procedures and
guidelines for verification and approval of EPD tools. Approval
number: NEPDT65.
Third party verifier:
Elisabet Amat, GREENIZE projects
(no signature required)
2 / 12
Product
Product description:
A net that is a complete bag of netting, used to contained farmed fish. The net consists primarily of netting and ropes. The ropes create the
structure and are designed to absorb the loads applied to the net.
Product specification
Components described in NS 9415 included: netting in polyamide, rope in PP and HDPE, Rope in polyamide and ABS, Thread in polyamide,
rundslings in polyester, centre ring in titanium, and copper based anti-fouling.
Components described in NS 9415 not included: floater, raft and anchoring.
Materials kg %
Metal - Titanium 1,70 0,06
Paint, water-based 585,00 20,22
Plastic net - Nylon 6 1683,00 58,16
Plastic rope - PP and HDPE 524,00 18,11
Plastic yarn - Nylon 6 96,47 3,33
Textile - Polyester (PE) 3,60 0,12
Total 2893,77
Packaging kg %
Packaging - Plastic 17,50 41,18
Packaging - Wood 25,00 58,82
Total incl. packaging 2936,27
Technical data:
ENC 160 1530 60: Straight-wall circular net. 160 indicates circumference. 1530 indicates depth measured from main rope to
bottom rope and to centre bottom. 60 indicates number of side ropes. The nets are produced according to the requirements of the Norwegian
Standard (NS) 9415 and the NYTEK Regulations.
Market:
Aquaculture
Reference service life, product
The validity period for a new net is 24 months. The product certificate’s validity period begins when the net
is placed in seawater, which must be no later than 12 months of the issue date. After 24 months, a net must have a supplemental valid service
history card. A service history card can extend the net’s validity period by a maximum of 24 months, provided that the net meets the required
durability and condition.
Reference service life, building or construction works
There is no standard service life for sea-based aquaculture farm. Each components have different service life and are repaired/replaced according
to the regulations in NS9415-2021.
LCA: Calculation rules
Declared unit:
1 pcs Enclosure ENC 160 1530 60
Cut-off criteria:
All major raw materials and all the essential energy is included. The production processes for raw materials and energy flows with very small
amounts (less than 1%) are not included. These cut-off criteria do not​ apply for hazardous materials and substances.
Allocation:
The allocation is made in accordance with the provisions of EN 15804. Incoming energy and water and waste production in-house is allocated
equally among all products through mass allocation. Effects of primary production of recycled materials is allocated to the main product in which
the material was used. The recycling process and transportation of the material is allocated to this analysis.
Data quality:
Specific data for the product composition are provided by the manufacturer. The data represent the production of the declared product and were
collected for EPD development in the year of study. Background data is based on EPDs according to EN 15804 and different LCA databases. The
data quality of the raw materials in A1 is presented in the table below.
3 / 12
Materials Source Data quality Year
Metal - Titanium ecoinvent 3.6 Database 2019
Packaging - Plastic ecoinvent 3.6 Database 2019
Paint, water-based ecoinvent 3.6 Database 2019
Packaging - Wood Modified ecoinvent 3.6 Database 2019
Textile - Polyester (PE) Modified ecoinvent 3.6 Database 2019
Company
Plastic rope - PP and HDPE Production data + ecoinvent 3.6 specific dataset 2021
+ database
Supplier data +
Plastic net - Nylon 6 Production data + ecoinvent 3.6 2021
database
Supplier data +
Plastic yarn - Nylon 6 Production data + ecoinvent 3.6 2021
database
4 / 12
System boundaries (X=included, MND=module not declared, MNR=module not relevant)
Construction Beyond the system
Product stage Use stage End of life stage
installation stage boundaries
A1 A2 A3 A4 A5 B1 B2 B3 B4 B5 B6 B7 C1 C2 C3 C4 D
X X X X MND MND MND MND MND MND MND MND X X X X X
System boundary:
Additional technical information:
waR slairetam tropsnarT gnirutcafunaM tropsnarT ylbmessA e​sU ecnanetniaM riapeR tnemecalpeR tnemhsibrufeR lanoitarepO ygrene esu lanoitarepO esu retaw -eD noitcurtsnoc noitilomed tropsnarT etsaW gnissecorp lasopsiD -yrevoceR-esueR laitnetop-gnilcyceR
5 / 12
LCA: Scenarios and additional technical information
The following information describe the scenarios in the different modules of the EPD.
Module A4 = a default travel distance of 300 km by truck is added to ensure distribution between the manufacturing site and the dock near the
production location at sea. In addition, a default travel distance of 1 Nm (1.852 km) of sea freight is added to cover the transport between the
dock and the production location at sea. Enclosures are transported onboard the vessel and not dragged in the sea.
Module C1 = deconstruction of the enclosure from the farm is estimated to require two hours of work boat aquaculture operations. In addition, a
default travel distance of 1 Nm (1.852 km) of sea freight is added to cover the transport between the production location at sea and the nearest
dock. Enclosures are transported onboard the vessel and not dragged in the sea.
Module C2 = a default travel distance of 300 km by truck is added to ensure transport between the dock and the waste treatment facility.
Modules C3 and C4 = Waste treatment of the product follows the default values provided in NPCR 031 part B for aquaculture infrastructure and
components, table 3. This table specified how different types of product categories and raw materials will likely be treated during the end-of-life
phases. Waste treatments in C3 include material recycling and incineration with and without energy recovery and fly ash extraction. Disposal in C4
consist of landfilling of different waste fractions and of ashes.
Module D = The recyclability of plastics and metals allows the producers a credit for the net scrap that is produced at the end of a product’s life.
The benefits from recycling of net scrap are described in formula from EN 15804:2012+A2:2019. Substitution of heat and electricity generated by
the incineration with energy recovery of plastics is also calculated in module D.
Capacity utilisation Value
Transport from production place to user (A4) Distance (km) Fuel/Energy Consumption Unit
(incl. return) % (Liter/tonne)
Ship, aquaculture transport, work boat, 14 meters,
20,0 % 2 1,790 l/tkm 3,32
without tugging (km) - Global
Truck, 16-32 tonnes, EURO 6 (km) - Europe 36,7 % 300 0,043 l/tkm 12,90
De-construction demolition (C1) Unit Value
Aquaculture operation, work boat, 14 meter,
h/DU 2,00
product de-construction (per hour) - Global
Ship, aquaculture transport, work boat, 14 meters,
kgkm/DU 5407,41
without tugging (kgkm) - Global
Capacity utilisation Value
Transport to waste processing (C2) Distance (km) Fuel/Energy Consumption Unit
(incl. return) % (Liter/tonne)
Truck, 16-32 tonnes, EURO 6 (km) - Europe 36,7 % 300 0,043 l/tkm 12,90
Waste processing (C3) Unit Value
Nylon 6 to recycling (kg) kg 996,50
Plastic compound, PP and HDPE, to recycling (kg) kg 366,80
Polyester to recycling (kg) kg 2,52
Titanium to recycling (kg) kg 1,53
Waste treatment of hazardous waste, incineration
kg 585,00
with energy recovery and fly ash extraction (kg)
Waste treatment of plastic mixture, incineration
kg 862,11
with energy recovery and fly ash extraction (kg)
Waste treatment per kg of impregnated
aquaculture components, washing process (kg) - kg 2893,77
Norway
Disposal (C4) Unit Value
Landfilling of ashes from incineration of
Hazardous waste, process per kg ashes and kg 110,57
residues (kg)
Landfilling of ashes from incineration of Plastic
kg 30,15
mixture, process per kg ashes and residues (kg)
Landfilling of plastic mixture (kg) kg 79,14
Landfilling of titanium (kg) kg 0,17
Benefits and loads beyond the system
Unit Value
boundaries (D)
Substitution of electricity, in Norway (MJ) MJ 1325,11
Substitution of polyamide, nylon 6, granulate (kg) kg 996,50
Substitution of polyethylene terephthalate, PET,
kg 2,52
amorphous (kg)
Substitution of Polyethylene, HDPE granulate (kg) kg 91,70
Substitution of Polypropylene, PP granulate (kg) kg 275,10
Substitution of primary titanium with net scrap
kg 1,29
(kg)
Substitution of thermal energy, district heating, in
MJ 20047,66
Norway (MJ)
6 / 12
LCA: Results
The LCA results are presented below for the declared unit defined on page 2 of the EPD document.
Environmental impact
Indicator Unit A1 A2 A3 A4 C1 C2 C3 C4 D
GWP-total kg CO2 -eq 2,95E+04 3,93E+02 1,48E+03 1,75E+02 1,99E+02 1,44E+02 4,18E+03 5,75E+01 -1,07E+04
GWP-fossil kg CO2 -eq 2,81E+04 3,93E+02 1,46E+03 1,75E+02 1,99E+02 1,44E+02 4,17E+03 5,74E+01 -1,07E+04
GWP-biogenic kg CO2 -eq 4,96E+01 1,45E-01 7,98E+00 6,57E-02 4,19E-02 5,96E-02 7,35E+00 2,00E-02 -1,28E+01
GWP-luluc kg CO2 -eq 1,40E+03 1,71E-01 4,79E+00 6,37E-02 9,06E-02 5,12E-02 1,91E+00 4,84E-03 -4,27E+00
ODP kg CFC11 -eq 1,44E-03 8,60E-05 2,56E-04 3,94E-05 4,32E-05 3,26E-05 2,49E-04 2,60E-06 -8,47E+00
AP mol H+ -eq 1,72E+02 4,62E+00 1,10E+01 1,49E+00 6,83E+00 4,14E-01 6,34E+00 1,02E-01 -3,99E+01
EP-FreshWater kg P -eq 6,81E-01 2,66E-03 2,23E-02 1,24E-03 6,00E-04 1,15E-03 5,22E-02 4,77E-04 -1,32E-01
EP-Marine kg N -eq 3,12E+01 1,11E+00 2,40E+00 3,42E-01 1,65E+00 8,18E-02 1,35E+00 3,65E-02 -9,07E+00
EP-Terrestial mol N -eq 2,82E+02 1,24E+01 2,71E+01 3,76E+00 1,80E+01 9,15E-01 1,55E+01 3,16E-01 -9,03E+01
POCP kg NMVOC -eq 9,57E+01 3,41E+00 7,53E+00 1,10E+00 4,74E+00 3,51E-01 4,80E+00 9,02E-02 -3,16E+01
ADP-minerals&metals1 kg Sb -eq 2,51E-01 8,42E-03 2,28E-02 4,12E-03 1,02E-03 3,97E-03 3,88E-02 8,83E-05 -7,35E-02
ADP-fossil1 MJ 3,83E+05 5,67E+03 2,29E+04 2,60E+03 2,71E+03 2,18E+03 1,77E+04 2,44E+02 -1,41E+05
WDP1 m3 3,59E+06 4,33E+03 7,57E+05 2,18E+03 4,76E+02 2,10E+03 8,48E+04 5,94E+03 -4,89E+04
GWP-total = Global Warming Potential total; GWP-fossil = Global Warming Potential fossil fuels; GWP-biogenic = Global Warming Potential biogenic; GWP-luluc =
Global Warming Potential land use and land use change; ODP = Depletion potential of the stratospheric ozone layer; AP = Acidification potential, Accumulated
Exceedance; EP-freshwater = Eutrophication potential, fraction of nutrients reaching freshwater end compartment: EP-marine = Eutrophication potential, fraction of
nutrients reaching marine end compartment; EP-terrestrial = Eutrophication potential, Accumulated Exceedance; POCP = Formation potential of tropospheric ozone;
ADP-minerals&metals = Abiotic depletion potential for non-fossil resources; ADP-fossil = Abiotic depletion for fossil resources potential; WDP = Water (user)
deprivation potential, deprivation-weighted water consumption
"Reading example: 9,0 E-03 = 9,0*10-3 = 0,009"
*INA Indicator Not Assessed
1. The results of this environmental impact indicator shall be used with care as the uncertainties on these results are high or as there is limited experienced with the
indicator
Remarks to environmental impacts
Risk of leaching hazardous materials to water: Antifouling is marked with the hazard statement H410: Very toxic to aquatic life with long lasting
effects.
Risk of plastic pollution: Ropes used for installing the net at sea must be cut, risk of ropes falling into the sea. Pay attention to this.
7 / 12
Additional environmental impact indicators
Indicator Unit A1 A2 A3 A4 C1 C2 C3 C4 D
PM Disease incidence 1,30E-03 2,01E-05 5,84E-05 1,63E-05 4,74E-05 8,81E-06 7,84E-05 7,71E-07 -4,23E-04
IRP2 kgBq U235 -eq 5,26E+02 2,47E+01 1,44E+02 1,14E+01 1,17E+01 9,51E+00 5,64E+01 1,35E+00 -2,76E+01
ETP-fw1 CTUe 2,06E+05 3,95E+03 1,72E+04 1,84E+03 1,46E+03 1,61E+03 4,63E+04 6,79E+02 -2,14E+04
HTP-c1 CTUh 2,20E-05 0,00E+00 5,52E-07 2,18E-08 1,53E-07 0,00E+00 2,63E-06 3,56E-08 -1,30E-06
HTP-nc1 CTUh 1,95E-04 4,43E-06 1,75E-05 1,96E-06 1,29E-06 1,76E-06 2,73E-05 1,30E-06 -3,04E-05
SQP1 dimensionless 1,50E+05 3,11E+03 1,22E+04 1,58E+03 3,53E+02 1,52E+03 9,43E+03 7,10E+02 -1,22E+04
PM = Particulate Matter emissions; IRP = Ionizing radiation – human health; ETP-fw = Eco toxicity – freshwater; HTP-c = Human toxicity – cancer effects; HTP-nc =
Human toxicity – non cancer effects; SQP = Potential Soil Quality Index (dimensionless)
"Reading example: 9,0 E-03 = 9,0*10-3 = 0,009"
*INA Indicator Not Assessed
1. The results of this environmental impact indicator shall be used with care as the uncertainties on these results are high or as there is limited experienced with the
indicator
2. This impact category deals mainly with the eventual impact of low dose ionizing radiation on human health of the nuclear fuel cycle. It does not consider effects due
to possible nuclear accidents, occupational exposure nor due to radioactive waste disposal in underground facilities. Potential ionizing radiation from the soil, from
radon and from some construction materials is also not measured by this indicator.
8 / 12
Resource use
Indicator Unit A1 A2 A3 A4 C1 C2 C3 C4 D
PERE MJ 4,41E+04 6,92E+01 1,68E+04 3,31E+01 1,34E+01 3,11E+01 5,76E+03 2,86E+01 -1,13E+04
PERM MJ 3,47E+02 0,00E+00 0,00E+00 0,00E+00 0,00E+00 0,00E+00 0,00E+00 0,00E+00 0,00E+00
PERT MJ 4,45E+04 6,92E+01 1,68E+04 3,31E+01 1,34E+01 3,11E+01 5,76E+03 2,86E+01 -1,13E+04
PENRE MJ 3,64E+05 5,67E+03 2,29E+04 2,60E+03 2,71E+03 2,18E+03 1,77E+04 2,44E+02 -1,29E+05
PENRM MJ 9,00E+04 0,00E+00 0,00E+00 0,00E+00 0,00E+00 0,00E+00 -8,95E+04 0,00E+00 -1,29E+04
PENRT MJ 3,85E+05 5,67E+03 2,29E+04 2,60E+03 2,71E+03 2,18E+03 -7,18E+04 2,44E+02 -1,42E+05
SM kg 1,13E+01 0,00E+00 0,00E+00 0,00E+00 0,00E+00 0,00E+00 0,00E+00 8,69E-03 -4,01E-01
RSF MJ 5,66E+02 2,38E+00 1,49E+02 1,11E+00 0,00E+00 1,11E+00 3,26E+01 5,21E-01 -2,37E+01
NRSF MJ 8,50E+01 7,71E+00 5,74E+01 3,98E+00 0,00E+00 3,98E+00 1,15E+02 5,10E+00 -6,11E+02
FW m3 3,17E+02 5,19E-01 1,06E+02 2,51E-01 1,22E-01 2,33E-01 4,52E+01 4,24E-01 -8,94E+01
PERE = Use of renewable primary energy excluding renewable primary energy resources used as raw materials; PERM = Use of renewable primary energy resources used
as raw materials; PERT = Total use of renewable primary energy resources; PENRE = Use of non renewable primary energy excluding non-renewable primary energy
resources used as raw materials; PENRM = Use of non renewable primary energy resources used as raw materials; PENRT = Total use of non renewable primary energy
resources; SM = Use of secondary materials; RSF = Use of renewable secondary fuels; NRSF = Use of non-renewable secondary fuels; FW = Net use of fresh water
"Reading example: 9,0 E-03 = 9,0*10-3 = 0,009"
*INA Indicator Not Assessed
9 / 12
End of life - Waste
Indicator Unit A1 A2 A3 A4 C1 C2 C3 C4 D
HWD kg 3,02E+01 2,76E-01 7,20E+00 1,25E-01 8,59E-02 1,12E-01 6,71E+02 8,02E-01 -1,59E+00
NHWD kg 3,85E+03 2,06E+02 4,73E+02 1,06E+02 4,21E+00 1,06E+02 8,43E+02 1,91E+02 -1,50E+02
RWD kg 5,71E-01 3,89E-02 1,24E-01 1,78E-02 1,91E-02 1,48E-02 3,64E-02 1,24E-04 -2,35E-02
HWD = Hazardous waste disposed; NHWD = Non-hazardous waste disposed; RWD = Radioactive waste disposed
"Reading example: 9,0 E-03 = 9,0*10-3 = 0,009"
*INA Indicator Not Assessed
End of life - Output flow
Indicator Unit A1 A2 A3 A4 C1 C2 C3 C4 D
CRU kg 0,00E+00 0,00E+00 0,00E+00 0,00E+00 0,00E+00 0,00E+00 0,00E+00 0,00E+00 0,00E+00
MFR kg 3,38E-02 0,00E+00 2,34E+01 0,00E+00 0,00E+00 0,00E+00 1,37E+03 7,10E-03 -2,17E-01
MER kg 7,33E-03 0,00E+00 5,13E-04 0,00E+00 0,00E+00 0,00E+00 1,45E+03 1,74E-04 -9,05E-01
EEE MJ 6,84E-02 0,00E+00 1,44E+01 0,00E+00 0,00E+00 0,00E+00 1,33E+03 1,13E-02 -1,51E+00
EET MJ 1,04E+00 0,00E+00 2,18E+02 0,00E+00 0,00E+00 0,00E+00 2,00E+04 1,70E-01 -2,29E+01
CRU = Components for re-use; MFR = Materials for recycling; MER = Materials for energy recovery; EEE = Exported energy electrical; EET = Exported energy thermal
"Reading example: 9,0 E-03 = 9,0*10-3 = 0,009"
*INA Indicator Not Assessed
Biogenic Carbon Content
Indicator Unit At the factory gate
Biogenic carbon content in product kg C 0,00E+00
Biogenic carbon content in accompanying packaging kg C 1,03E+01
Note: 1 kg biogenic carbon is equivalent to 44/12 kg CO2
10 / 12
Additional requirements
Greenhouse gas emissions from the use of electricity in the manufacturing phase
National production mix from import, low voltage (production of transmission lines, in addition to direct emissions and losses in grid) of applied
electricity for the manufacturing process (A3).
Electricity mix Data source Amount Unit
Electricity, Lithuania (kWh) ecoinvent 3.6 373,46 g CO2-eq/kWh
Electricity, Norway (kWh) ecoinvent 3.6 24,33 g CO2-eq/kWh
Dangerous substances
The product contains no substances given by the REACH Candidate list.
Indoor environment
Additional Environmental Information
Additional environmental impact indicators required in NPCR Part A for construction products
Indicator Unit A1 A2 A3 A4 C1 C2 C3 C4 D
GWPIOBC kg CO2 -eq 2,96E+04 3,93E+02 1,57E+03 1,75E+02 1,99E+02 1,44E+02 4,18E+03 5,09E+01 -1,07E+04
GWP-IOBC: Global warming potential calculated according to the principle of instantaneous oxidation. In order to increase the transparency of biogenic carbon​
contribution to climate impact, the indicator GWP-IOBC is required as it declares climate impacts calculated according to the principle of instantaneous oxidation.​
GWP-IOBC is also referred to as GWP-GHG in context to Swedish public procurement legislation.
11 / 12
Bibliography
ISO 14025:2010. Environmental labels and declarations - Type III environmental declarations - Principles and procedures. International
Organization for Standardization.
ISO 14044:2006. Environmental management - Life cycle assessment - Requirements and guidelines. International Organization for
Standardization.
EN 15804:2012+A2:2019. Environmental product declaration - Core rules for the product category of construction products. European
Committee for Standardization.
ISO 21930:2017. Sustainability in buildings and civil engineering works - Core rules for environmental product declarations of construction
products. International Organization for Standardization.
Ecoinvent v3, 2019. Allocation, cut-off by classification. Swiss Centre of Life Cycle Inventories.
Iversen et al., (2021). eEPD v2021.09, background information for EPD generator tool system verification, LCA.no. Report number: 07.21. System
verification report.
Gaspard Philis (2023). EPD generator for NPCR 031 part B for aquaculture infrastructure and components, Background information for EPD
generator application and LCA data, LCA.no report number: 03.23. PCR verification report.
EPD Norway (2022). NPCR Part A: Construction products and services. The Norwegian EPD foundation. Version 2.0 published 24.03.2021.
EPD Norway (2023). NPCR 031 Part B for aquaculture infrastructure and components. The Norwegian EPD foundation. Version 1.0 published
26.04.2023.
Program operator and publisher Phone: +47 23 08 80 00
The Norwegian EPD Foundation e-mail: post@epd-norge.no
Post Box 5250 Majorstuen, 0303 Oslo, Norway web: www.epd-norge.no
Owner of the declaration: Phone: +47 91557400
AKVA group ASA e-mail: tolafsen@akvagroup.com
Plogfabrikkvegen 11, 4353 Klepp Stasjon web: https://www.akvagroup.com
Author of the Life Cycle Assessment Phone: +47 916 50 916
LCA.no AS e-mail: post@lca.no
Dokka 6B, 1671 web: www.lca.no
Developer of EPD generator Phone: +47 916 50 916
LCA.no AS e-mail: post@lca.no
Dokka 6B,1671 Kråkerøy web: www.lca.no
ECO Platform web: www.eco-platform.org
ECO Portal web: ECO Portal
12 / 12
