Environmental product declaration
In accordance with 14025 and EN15804+A2
NOIKLX 90 3G1,5
Owner of the declaration: Program operator:
NKT A/S The Norwegian EPD Foundation
Product: Declaration number:
NOIKLX 90 3G1,5
Registration number:
Declared unit:
1 m Issue date:
This declaration is based on Product Category Rules: Valid to:
CEN Standard EN 15804:2012+A2:2019 serves as core
EPD Software:
PCR
The Norwegian EPD Foundation LCA.no EPD generator ID: 56947
NPCR 027 Part B for Electrical cables and wires
1 / 12
General information
Product Owner of the declaration:
NOIKLX 90 3G1,5 NKT A/S
Contact person: Matheo Roehr
Phone:
e-mail: matheo.roehr@nkt.com
Program operator: Manufacturer:
Post Box 5250 Majorstuen, 0303 Oslo, Norway NKT A/S
The Norwegian EPD Foundation Vibeholms Allé 20
Phone: +47 23 08 80 00 2605 Brøndby, Denmark
web: post@epd-norge.no
Declaration number: Place of production:
NKT production site Warszowice (Poland)
Gajowa 3
43-254 Warszowice, Poland
This declaration is based on Product Category Rules: Management system:
CEN Standard EN 15804:2012+A2:2019 serves as core PCR ISO 9001, ISO 14001
NPCR 027 Part B for Electrical cables and wires
Statement of liability: Organisation no:
The owner of the declaration shall be liable for the underlying 957 338 690
information and evidence. EPD Norway shall not be liable with respect
to manufacturer information, life cycle assessment data and
evidences.​
Declared unit: Issue date:
1 m NOIKLX 90 3G1,5
Declared unit with option: Valid to:
A1,A2,A3,A4,A5,C1,C2,C3,C4,D
Year of study:
2021
Functional unit: Comparability:
1 m of NOIKLX 90 3G1,5 installed electrical cable used to transmit a EPD of construction products may not be comparable if they not
reference electric current of 1A over 30 years, including waste comply with EN 15804 and seen in a building context.
treatment at end-of-life.
General information on verification of EPD from EPD tools: Development and verification of EPD:
Independent verification of data, other environmental information The declaration is created using EPD tool lca.tools ver EPD2022.03,
and the declaration according to ISO 14025:2010, § 8.1.3 and § 8.1.4. developed by LCA.no. The EPD tool is integrated in the company's
Individualthird party verification of each EPD is not required when the management system, and has been approved by EPD Norway.
EPD tool is i) integrated into the company's environmental Approval number:
management system, ii) the procedures for use of the EPD tool are
approved by EPDNorway, and iii)the proccess is reviewed annualy. See Developer of EPD: Ann Aittamaa
Appendix G of EPD-Norway's General Programme Instructions for
Reviewer of company-specific input data and EPD:​ Matheo Roehr
further information on EPD tools.
Verification of EPD tool: Approved:
Independent third party verification of the EPD tool, background data
and test-EPD in accordance with EPDNorway's procedures and
guidelines for verification and approval of EPD tools. Approval
number: NEPDT32.
Third party verifier:
Vito D’Incognito - Take Care International
(no signature required)
2 / 12
Product
Product description:
Where halogen-free and environmentally friendly cables are required. For fixed installation in dry and wet rooms and outside as well as in the
open air. Can be laid in the ground. May be bricked in and embedded directly. Not suitable for embedment in vibrated concrete. Conductor
insulation must be protected against light exposure. Installation to be performed by a licensed electrician only.
Product specification
Conductor:
1,5-4 mm2: Copper conductor, solid cl. 1
6-50 mm2: Copper conductor, stranded cl. 2
PEX insulation:
1,5-2,5 mm2: Filling sheath, thermoplastic compound
> 4 mm2: EPDM-rubber
Outer sheath:
Thermoplastic compound, UV-stabilized
Materials kg %
HFFR Polyolefin 0,04 46,57
Metal - Copper 0,04 44,05
Plastic - Polyethylene 0,01 9,38
Total 0,09
Technical data:
NOIKLX 90 3G1,5
Standard applied: NKT factory standard no. 008
Rated voltage: 300/500V
Test voltage: 2 kV AC
Operating temperature: 90°C
Conductor temperature: 90 °C
Max. short-circuit temperature: 250 °C
Min. handling temperature: -15 °C
Max. storage temperature: 40 °C
Color of the sheath: Light grey
Smoke density: IEC 61034
Fire test: IEC 60332-1
CPR fire class: Eca
Emission of corrosive gases: IEC 60754-1, EN 50267-2-1
Conductivity - pH change: IEC 60754-2, EN 50267-2-3
Min. bending radius:
1-5 core (1,5-2,5mm2): 5 x cable diameter
Multi-core (>2,5 mm2): 8 x cable diameter
1-core (>2,5 mm2): 10 x cable diameter
Max. pulling force: 50 N/mm2 on conductors
CE-conformity: Low Voltage Directive
Market:
Denmark
Reference service life, product
30 years. As defined in appendix 1 of the PEP Ecopassport PSR.
Reference service life, building or construction works
30 years.
LCA: Calculation rules
Declared unit:
1 m NOIKLX 90 3G1,5
Cut-off criteria:
All major raw materials and all the essential energy is included. The production processes for raw materials and energy flows with very small
amounts (less than 1%) are not included. These cut-off criteria do not apply for hazardous materials and substances.
3 / 12
Allocation:
The allocation is made in accordance with the provisions of EN 15804. Incoming energy and water and waste production in-house is allocated
equally among all products through mass allocation. Effects of primary production of recycled materials is allocated to the main product in which
the material was used. The recycling process and transportation of the material is allocated to this analysis.
Data quality:
Specific data for the product composition are provided by the manufacturer. The data represent the production of the declared product and were
collected for EPD development in the year of study. Background data is based on EPDs according to EN 15804 and different LCA databases. The
data quality of the raw materials in A1 is presented in the table below.
Materials Source Data quality Year
HFFR Polyolefin ecoinvent 3.6 Database 2019
Metal - Copper ecoinvent 3.6 Database 2019
Plastic - Polyethylene ecoinvent 3.6 Database 2019
4 / 12
System boundaries (X=included, MND=module not declared, MNR=module not relevant)
Construction Beyond the system
Product stage Use stage End of life stage
installation stage boundaries
A1 A2 A3 A4 A5 B1 B2 B3 B4 B5 B6 B7 C1 C2 C3 C4 D
X X X X X MND MND MND MND MND MND MND X X X X X
System boundary:
The flowchart below illustrates the system boundaries of the analysis:
Additional technical information:
The reference product NOIKLX 90 3G1,5 represents the entire product family.
Please contact us for a specific EPD of another cable in the product family:
3G1,5 Rg 50 30 33 778 005
3G1,5 QB 75 30 33 779 538
3G1,5 Rg 100 30 33 778 018
3G1,5 QA 500 30 33 779 101
4G1,5 RG 100 30 33 778 050
5G1,5 QB 50 30 33 779 554
5G1,5 Rg 50 30 33 778 186
5G1,5 Rg 100 30 33 778 199
5G1,5 QA 450 30 33 779 127
7G1,5 Rg 50 30 33 779 350
7G1,5 Rg 100 30 33 779 363
7G1,5 QA 400 30 33 779 143
10G1,5 Tr 500 30 33 778 335
14G1,5 Tr 500 30 33 778 393
19G1,5 Tr 500 30 33 778 403
27G1,5 Tr 500 30 33 778 416
37G1,5 Tr 500 30 33 778 432
1G2,5 Rg 100 30 33 778 571
1G2,5 QA 500 30 33 779 185
3G2,5 Rg 50 30 33 778 584
3G2,5 Rg 100 30 33 778 597
waR slairetam tropsnarT gnirutcafunaM tropsnarT ylbmessA e​sU ecnanetniaM riapeR tnemecalpeR tnemhsibrufeR lanoitarepO ygrene esu lanoitarepO esu retaw -eD noitcurtsnoc noitilomed tropsnarT etsaW gnissecorp lasopsiD -yrevoceR-esueR laitnetop-gnilcyceR
5 / 12
LCA: Scenarios and additional technical information
The following information describe the scenarios in the different modules of the EPD.
Module A4 = An average distance between the factory and the market is considered.
Modules A5 = 2 % product losses during installation are estimated by the company. No energy use for installation has been quantified since this
operation is assumed to be done with other products and should be assessed at a construction works level. Cable drums are reused and assumed
under the cut-off criterion of 1%.
Module C1 = For both buildings and construction works, cables will be taken out as part of a larger demolition. The energy use for cable removal
compared to other heavier materials is assumed to be low. This module can therefore be included with zero impact.
Module C2 = An average distance between the market and the waste treatment facility is considered.
Modules C3 and C4 = Waste treatment of the product follows the default values provided in EN 50693, Product Category Rules for life cycle
assessments of electronic and electrical products and systems, table G.4. This table specified how different types of raw materials used in A1 will
likely be treated during the end-of-life of the product. Waste treatments in C3 include material recycling and incineration with and without energy
recovery and fly ash extraction. Disposal in C4 consist of landfilling of different waste fractions and of ashes.
Module D = The recyclability of metals and plastics allows the producers a credit for the net scrap that is produced at the end of a product’s life.
The benefits from recycling of net scrap are described in formula from EN 15804:2012+A2:2019. Substitution of heat and electricity generated by
the incineration with energy recovery of plastic insulation and other parts is also calculated in module D.
Capacity utilisation Value
Transport from production place to user (A4) Distance (km) Fuel/Energy Consumption Unit
(incl. return) % (Liter/tonne)
Truck, over 32 tonnes, EURO 6 (km) - Europe 53,3 % 1210 0,023 l/tkm 27,83
Assembly (A5) Unit Value
Product loss during installation (percentage of
Units/DU 0,02
cable)
Capacity utilisation Value
Transport to waste processing (C2) Distance (km) Fuel/Energy Consumption Unit
(incl. return) % (Liter/tonne)
Truck, over 32 tonnes, EURO 6 (km) - Europe 53,3 % 300 0,023 l/tkm 6,90
Waste processing (C3) Unit Value
Copper to recycling (kg) kg 0,02
Waste treatment of plastic mixture, incineration
kg 0,02
with energy recovery and fly ash extraction (kg)
Waste treatment of polyethylene (PE),
incineration with energy recovery and fly ash kg 0,00
extraction (kg)
Disposal (C4) Unit Value
Landfilling of ashes from incineration of Plastic
kg 0,00
mixture, process per kg ashes and residues (kg)
Landfilling of ashes from incineration of
Polyethylene (PE), process per kg ashes and kg 0,00
residues (kg)
Landfilling of copper (kg) kg 0,02
Landfilling of plastic mixture (kg) kg 0,02
Benefits and loads beyond the system
Unit Value
boundaries (D)
Substitution of electricity, in Norway (MJ) MJ 0,04
Substitution of primary copper with net scrap (kg) kg 0,02
Substitution of thermal energy, district heating, in
MJ 0,59
Norway (MJ)
6 / 12
LCA: Results
The LCA results are presented below for the declared unit defined on page 2 of the EPD document.
Environmental impact
Indicator Unit A1 A2 A3 A4 A5 C1 C2 C3 C4 D
GWP-total
kg CO2 -
3,55E-01 6,73E-03 3,68E-03 9,39E-03 8,81E-03 0 2,33E-03 6,05E-02 3,02E-03 -4,52E-02
eq
GWP-fossil
kg CO2 -
3,50E-01 6,73E-03 3,36E-03 9,38E-03 8,71E-03 0 2,33E-03 6,05E-02 3,02E-03 -4,48E-02
eq
GWP-biogenic
kg CO2 -
4,40E-03 2,88E-06 3,01E-04 4,02E-06 9,42E-05 0 9,96E-07 1,15E-06 2,54E-07 -2,00E-04
eq
GWP-luluc
kg CO2 -
2,71E-04 2,05E-06 2,23E-05 2,86E-06 5,99E-06 0 7,09E-07 2,10E-07 1,42E-07 -1,62E-04
eq
kg
ODP CFC11 - 4,93E-06 1,62E-09 6,56E-10 2,26E-09 9,87E-08 0 5,61E-10 1,14E-10 1,40E-10 -2,51E-04
eq
mol H+
AP 9,20E-03 2,17E-05 6,53E-05 3,02E-05 1,87E-04 0 7,49E-06 1,21E-05 3,64E-06 -6,98E-03
-eq
EP-FreshWater kg P -eq 7,26E-05 5,35E-08 2,02E-07 7,46E-08 1,46E-06 0 1,85E-08 1,02E-08 6,65E-09 -4,72E-05
EP-Marine kg N -eq 7,04E-04 4,74E-06 1,98E-05 6,61E-06 1,49E-05 0 1,64E-06 5,79E-06 4,21E-06 -2,95E-04
mol N -
EP-Terrestial 9,91E-03 5,29E-05 3,13E-04 7,38E-05 2,09E-04 0 1,83E-05 5,98E-05 1,46E-05 -4,53E-03
eq
kg
POCP NMVOC 2,61E-03 2,08E-05 5,61E-05 2,90E-05 5,48E-05 0 7,18E-06 1,44E-05 4,73E-06 -1,23E-03
-eq
ADP- kg Sb -
8,20E-05 1,20E-07 3,02E-08 1,67E-07 1,65E-06 0 4,14E-08 5,70E-09 3,59E-09 -3,90E-05
minerals&metals1 eq
ADP-fossil1 MJ 5,60E+00 1,09E-01 3,09E-02 1,52E-01 1,19E-01 0 3,78E-02 7,43E-03 1,08E-02 -4,19E-01
WDP1 m3 1,85E+01 8,38E-02 2,51E-02 1,17E-01 3,80E-01 0 2,90E-02 4,96E-02 1,80E-01 1,65E+00
GWP total Global Warming Potential total; GWP fossil Global Warming Potential fossil fuels ; GWP biogenic Global Warming Potential biogenic; GWP luluc Global W
Potential land use change; ODP Ozone Depletion; AP Acidification; EP freshwater Eutrophication aquatic freshwater; EP marine Eutrophication aquatic marine; EP
terrestrial Eutrophication terrestrial ;POCP Photochemical zone formation; ADPE Abiotic Depletion Potential minerals and metals; ADPf Abiotic Depletion Potential fossil
fuels;
"Reading example: 9,0 E-03 = 9,0*10-3 = 0,009"
*INA Indicator Not Assessed
1. The results of this environmental impact indicator shall be used with care as the uncertainties on these results are high or as there is limited experienced with the
indicator
Remarks to environmental impacts
7 / 12
Additional environmental impact indicators
Indicator Unit A1 A2 A3 A4 A5 C1 C2 C3 C4 D
PM Disease incidence 3,12E-08 6,18E-10 9,03E-10 8,62E-10 6,78E-10 0 2,14E-10 5,20E-11 6,80E-11 -1,56E-08
IRP2 kgBq U235 -eq 1,63E-02 4,78E-04 1,14E-04 6,66E-04 3,56E-04 0 1,65E-04 1,80E-05 6,17E-05 -7,74E-04
ETP-fw1 CTUe 1,08E+02 7,99E-02 5,92E-01 1,11E-01 2,37E+00 0 2,76E-02 1,04E-01 9,54E+00 -6,42E+01
HTP-c1 CTUh 1,97E-09 0,00E+00 7,00E-12 0,00E+00 4,00E-11 0 0,00E+00 3,00E-12 0,00E+00 -9,07E-10
HTP-nc1 CTUh 1,45E-07 7,80E-11 2,01E-10 1,08E-10 2,92E-09 0 2,70E-11 1,37E-10 1,30E-11 -7,76E-08
SQP1 dimensionless 2,64E+00 1,25E-01 2,39E+00 1,75E-01 1,08E-01 0 4,33E-02 1,31E-03 3,04E-02 -1,14E+00
PM Particulate Matter emissions; IRP Ionizing radiation – human health; ETP-fw Eco toxicity – freshwater; HTP-c Human toxicity – cancer effects; HTP-nc Human
toxicity – non cancer effects; SQP Soil Quality (dimensionless)
"Reading example: 9,0 E-03 = 9,0*10-3 = 0,009"
*INA Indicator Not Assessed
1. The results of this environmental impact indicator shall be used with care as the uncertainties on these results are high or as there is limited experienced with the
indicator
2. This impact category deals mainly with the eventual impact of low dose ionizing radiation on human health of the nuclear fuel cycle. It does not consider effects due
to possible nuclear accidents, occupational exposure nor due to radioactive waste disposal in underground facilities. Potential ionizing radiation from the soil, from
radon and from some construction materials is also not measured by this indicator.
8 / 12
Resource use
Indicator Unit A1 A2 A3 A4 A5 C1 C2 C3 C4 D
PERE MJ 7,36E-01 1,37E-03 5,00E-01 1,92E-03 2,48E-02 0 4,75E-04 3,92E-04 9,78E-04 -4,52E-01
PERM MJ 0,00E+00 0,00E+00 0,00E+00 0,00E+00 0,00E+00 0 0,00E+00 0,00E+00 0,00E+00 0,00E+00
PERT MJ 7,36E-01 1,37E-03 5,00E-01 1,92E-03 2,48E-02 0 4,75E-04 3,92E-04 9,78E-04 -4,52E-01
PENRE MJ 4,54E+00 1,09E-01 3,10E-02 1,52E-01 9,77E-02 0 3,78E-02 7,43E-03 1,08E-02 -4,19E-01
PENRM MJ 1,09E+00 0,00E+00 0,00E+00 0,00E+00 1,04E-03 0 0,00E+00 -1,04E+00 0,00E+00 0,00E+00
PENRT MJ 5,63E+00 1,09E-01 3,10E-02 1,52E-01 9,88E-02 0 3,78E-02 -1,04E+00 1,08E-02 -4,19E-01
SM kg 6,66E-03 0,00E+00 1,32E-06 0,00E+00 1,35E-04 0 0,00E+00 0,00E+00 7,96E-05 1,21E-02
RSF MJ 1,87E-02 4,81E-05 1,91E-05 6,70E-05 3,78E-04 0 1,66E-05 8,59E-06 2,03E-05 1,10E-03
NRSF MJ 1,36E-03 1,61E-04 1,12E-04 2,25E-04 3,87E-05 0 5,57E-05 0,00E+00 1,91E-05 -1,55E-02
FW m3 6,65E-03 1,24E-05 1,58E-05 1,73E-05 1,35E-04 0 4,30E-06 5,83E-05 1,38E-05 -1,38E-03
PERE Use of renewable primary energy excluding renewable primary energy resources used as raw materials; PERM Use of renewable primary energy resources used as
raw materials; PERT Total use of renewable primary energy resources; PENRE Use of non renewable primary energy excluding non-renewable primary energy resources
used as raw materials; PENRM Use of non renewable primary energy resources used as raw materials; PENRT Total use of non renewable primary energy resources; SM
Use of secondary materials; RSF Use of renewable secondary fuels; NRSF Use of non renewable secondary fuels; FW Use of net fresh water
"Reading example: 9,0 E-03 = 9,0*10-3 = 0,009"
*INA Indicator Not Assessed
9 / 12
End of life - Waste
Indicator Unit A1 A2 A3 A4 A5 C1 C2 C3 C4 D
HWD kg 1,90E-03 5,98E-06 5,01E-04 8,34E-06 6,27E-05 0 2,07E-06 0,00E+00 7,19E-04 -4,71E-04
NHWD kg 1,15E-01 9,50E-03 1,29E-03 1,32E-02 3,65E-03 0 3,28E-03 0,00E+00 4,02E-02 -2,11E-02
RWD kg 1,55E-05 7,46E-07 1,74E-07 1,04E-06 3,55E-07 0 2,58E-07 0,00E+00 7,32E-08 -6,73E-07
HWD = Hazardous waste disposed; NHWD = Non-hazardous waste disposed; RWD = Radioactive waste disposed;
"Reading example: 9,0 E-03 = 9,0*10-3 = 0,009"
*INA Indicator Not Assessed
End of life - Output flow
Indicator Unit A1 A2 A3 A4 A5 C1 C2 C3 C4 D
CRU kg 0,00E+00 0,00E+00 0,00E+00 0,00E+00 0,00E+00 0 0,00E+00 0,00E+00 0,00E+00 0,00E+00
MFR kg 1,09E-05 0,00E+00 4,20E-05 0,00E+00 4,63E-04 0 0,00E+00 2,31E-02 2,34E-06 -4,74E-04
MER kg 2,55E-05 0,00E+00 2,01E-08 0,00E+00 4,90E-04 0 0,00E+00 2,45E-02 2,00E-06 -6,24E-05
EEE MJ 4,74E-05 0,00E+00 1,03E-03 0,00E+00 8,06E-04 0 0,00E+00 3,92E-02 2,07E-05 -1,53E-04
EET MJ 7,17E-04 0,00E+00 1,56E-02 0,00E+00 1,22E-02 0 0,00E+00 5,93E-01 3,14E-04 -2,31E-03
CRU = Components for re-use; MFR = Materials for recycling; MER = Materials for energy recovery; EEE = Exported electrical energy; EET = Exported energy ​ Thermal
"Reading example: 9,0 E-03 = 9,0*10-3 = 0,009"
*INA Indicator Not Assessed
Biogenic Carbon Content
Indicator Unit At the factory gate
Biogenic carbon content in product kg C 0,00E+00
Biogenic carbon content in accompanying packaging kg C 0,00E+00
Note: 1 kg biogenic carbon is equivalent to 44/12 kg CO2
10 / 12
Additional Norwegian requirements
Greenhouse gas emissions from the use of electricity in the manufacturing phase
National production mix from import, low voltage (production of transmission lines, in addition to direct emissions and losses in grid) of applied
electricity for the manufacturing process (A3).
Electricity mix Data source Amount Unit
Electricity, renewable with guarantee of origin, low voltage, Poland (kWh) - NKT ecoinvent 3.6 71,22 g CO2-eq/kWh
Dangerous substances
The product contains no substances given by the REACH Candidate list or the Norwegian priority list.
Indoor environment
Additional Environmental Information
Environmental impact indicators EN 15804+A1 and NPCR Part A v2.0
Indicator Unit A1 A2 A3 A4 A5 C1 C2 C3 C4 D
GWP kg CO2 -eq 3,40E-01 6,66E-03 3,48E-03 9,29E-03 8,50E-03 0 2,30E-03 6,05E-02 2,42E-03 -4,35E-02
ODP kg CFC11 -eq 6,57E-06 1,31E-09 6,32E-10 1,83E-09 1,31E-07 0 4,54E-10 1,06E-10 1,19E-10 -2,08E-09
POCP kg C2H4 -eq 3,35E-04 8,24E-07 2,79E-06 1,15E-06 6,81E-06 0 2,85E-07 1,68E-07 4,66E-07 -2,35E-04
AP kg SO2 -eq 7,31E-03 1,40E-05 3,89E-05 1,96E-05 1,48E-04 0 4,85E-06 8,46E-06 1,51E-06 -5,96E-03
EP kg PO43- -eq 4,21E-04 1,52E-06 1,30E-05 2,12E-06 8,84E-06 0 5,26E-07 2,83E-06 1,55E-06 -2,55E-04
ADPM kg Sb -eq 8,20E-05 1,20E-07 3,02E-08 1,67E-07 1,65E-06 0 4,14E-08 5,70E-09 3,83E-09 -3,90E-05
ADPE MJ 4,91E+00 1,07E-01 3,03E-02 1,50E-01 1,05E-01 0 3,71E-02 7,43E-03 1,02E-02 -4,19E-01
GWPIOBC kg CO2 -eq 3,54E-01 6,73E-03 2,46E-03 9,39E-03 8,71E-03 0 2,33E-03 6,05E-02 3,34E-04 -2,32E-02
GWP Global warming potential; ODP Depletion potential of the stratospheric ozone layer; POCP Formation potential of tropospheric photochemical oxidants; AP
Acidification potential of land and water; EP Eutrophication potential; ADPM Abiotic depletion potential for non fossil resources; ADPE Abiotic depletion​ potential for
fossil resources; GWP-IOBC/GHG Global warming potential calculated according to the principle of instantanious oxidation (except emissions and uptake of biogenic
carbon)
11 / 12
Bibliography
ISO 14025:2010. Environmental labels and declarations - Type III environmental declarations - Principles and procedures. International
Organization for Standardization.
ISO 14044:2006. Environmental management - Life cycle assessment - Requirements and guidelines. International Organization for
Standardization.
EN 15804:2012+A2:2019. Environmental product declaration - Core rules for the product category of construction products. European
Committee for Standardization.
ISO 21930:2017. Sustainability in buildings and civil engineering works - Core rules for environmental product declarations of construction
products. International Organization for Standardization.
EN 50693:2019. Product category rules for life cycle assessments of electronic and electrical products and systems. European Committee for
Standardization.
Ecoinvent v3, 2019. Allocation, cut-off by classification. Swiss Centre of Life Cycle Inventories.
Iversen et al., (2021). eEPD v2021.09, background information for EPD generator tool system verification, LCA.no. Report number: 07.21. System
verification report.
Philis et al., (2022). EPD generator for NPCR 027 part B for electrical wires and cables, background information for EPD generator application and
LCA data, LCA.no Report number: 03.22. PCR verification report.
EPD Norway (2022). NPCR Part A: Construction products and services. The Norwegian EPD foundation. Version 2.0 published 24.03.2021.
EPD Norway (2022). NPCR 027 Part B for electrical cables and wires. The Norwegian EPD foundation. Version 2.0 published 01.03.2022.
Program operator and publisher Phone: +47 23 08 80 00
The Norwegian EPD Foundation e-mail: post@epd-norge.no
Post Box 5250 Majorstuen, 0303 Oslo, Norway web: www.epd-norge.no
Owner of the declaration: Phone:
NKT A/S e-mail: matheo.roehr@nkt.com
Vibeholms Allé 20, 2605 Brøndby web: nkt.com
Author of the Life Cycle Assessment Phone: +47 916 50 916
LCA.no AS e-mail: post@lca.no
Dokka 6B, 1671 web: www.lca.no
Developer of EPD generator Phone: +47 916 50 916
LCA.no AS e-mail: post@lca.no
Dokka 6B,1671 Kråkerøy web: www.lca.no
ECO Platform web: www.eco-platform.org
ECO Portal web: ECO Portal
12 / 12
