ENVIRONMENTAL PRODUCT DECLARATION
In accordance with ISO 14025 and EN 15804+A2
Beyer Baustoffhandelsgesellsch. mbH – WU-Beton C30/37 XC4, XD1, XF1, XM1,
XA1; Dmax=32mm
Owner of the declaration Program operator:
Beyer Baustoffhandelsgesellsch. mbH EPD-Norge
Robert-Koch-Str. 32 Majorstuen P.O. Box 5250
55129 Mainz - Hechtsheim N-0303 Oslo
Germany Norway
Product Declaration number:
WU-Beton C30/37 XC4, XD1, XF1, XM1, XA1; NEPD-7701-7040-2
Dmax=32mm
Registration number:
Declared product / Declared unit NEPD-7701-7040-2
1 m³ of WU-Beton C30/37 XC4, XD1, XF1,
Issue date
XM1, XA1; Dmax=32mm
02.10.2024
This declaration is based on Product
Valid to
Category Rules
02.10.2029
EN 15804:2012 + A2:2019,
NPCR 020 PART B for concrete and concrete EPD Software
elements (v3.0) Emidat EPD Tool v1.0.0
EPD for the best environmental decision 1
General Information
Product Contact person
WU-Beton C30/37 XC4, XD1, XF1, XM1, XA1; Dmax=32mm Oliver Juli
Program Operator Phone
EPD-Norge +49 6131 9179 114
Majorstuen P.O. Box 5250
Email
N-0303 Oslo
Oliver.Juli@beyer-baustoffe.de
Norway
Phone: +47 23 08 80 00
Manufacturer
Email: post@epd-norge.no
Beyer Baustoffhandelsgesellsch. mbH
Robert-Koch-Str. 32
Declaration Number
55129 Mainz - Hechtsheim, Germany
NEPD-7701-7040-2
Place of production
This declaration is based on Product Category Rules
Mainz, Germany
EN 15804:2012 + A2:2019,
NPCR 020 PART B for concrete and concrete elements
Management system
(v3.0)
-
Statements
Organisation no
The owner of the declaration shall be liable for the
HRB 2891
underlying information and evidence. EPD Norway shall not
be liable with respect to manufacturer, life cycle Issue date
assessment data and evidences. 02.10.2024
Declared unit Valid to
1 m³ of WU-Beton C30/37 XC4, XD1, XF1, XM1, XA1; 02.10.2029
Dmax=32mm
Year of study
General information on verification of EPD from EPD 2023
tools
Comparability
Independent verification of data, other environmental
EPDs of construction products may not be comparable if
information and the declaration according to ISO
they do not comply with EN 15804 and are not seen in a
14025:2010, § 8.1.3 and § 8.1.4.
building context. EPD data may not be comparable if the
Verification of each EPD is made according to EPD-
datasets used are not developed in accordance with EN
Norway's guidelines for verification and approval requiring
15804 and if the background systems are not based on the
that tools are i) integrated into the company's
same database (including primary and secondary data).
environmental management system, ii) the procedures for
use of the EPD tool are approved by EPD-Norway, and iii)
Development and verification of EPD
the process is reviewed annually by an independent third
The declaration was created using the Emidat EPD tool
party verifier. See Appendix G of EPD-Norway's General
v1.0, developed by Emidat GmbH. The EPD tool is
Programme Instructions for further information on EPD
integrated in the company's management system, and has
tools.
been approved by EPD Norway.
Developer of EPD: Oliver Juli
Verification of EPD tool
Reviewer of company-specific input data and EPD: Jeanette
Charlotte Merlin, FORCE Technology
Müller
(no signature required)
Approved
Owner of the declaration
Beyer Baustoffhandelsgesellsch. mbH
Håkon Hauan, CEO EPD-Norge
EPD for the best environmental decision 2
Product
Product description
Concrete is a building material made up of several components, including cement, water, sand, gravel, and air. Ready-mix
concrete is manufactured in a batch plant in a controlled environment, using precise mix designs (with the addition of other
cementitious materials or chemical admixtures that improve the properties of the concrete), ensuring consistency in quality,
strength, and composition. This consistency leads to predictable performance in construction projects. Ready-mix concrete is
then delivered to the construction site in an unhardened state, ready to use, eliminating the need for on-site mixing. This
saves time in labor, equipment setup, and material handling, speeding up the construction process. The product is produced
according to DIN EN 206. Testing was conducted according to EN 12350 and EN 12390. Performance data of the product with
respect to its characteristics in accordance with the relevant technical provision (no CE-marking).
🪨 Admixtures
🪨 Cement
WU-Beton
🪨 Fly ash C30/37 XC4,
Mixing and
🪨 Natural blending XD1, XF1,
aggregates XM1, XA1;
Dmax=32mm
🪨 Sand
🪨 Water
The most common man-made substance in the world is concrete. Regardless of the magnitude of the construction, it is a
necessary component of roads, buildings, bridges, dams, pavements, pipelines, sewers, and other structures. It is made up of
naturally occurring aggregates with varying granulometries (sand, fine gravel, and gravel) joined by hydrated cement paste.
To improve particular qualities of the fresh or hardened concrete, such as workability, durability, or early and final strength,
chemical admixtures can also be used. After manufacture, concrete is workable enough to be transported, poured, pumped,
put in place, and compacted at the project site, where it gradually solidifies and gains strength.
Product specification
Name of ingredient Share of total weight Country of origin
Admixtures 0 - 2 % Germany
Cement 10 - 25 % Germany
Fly ash 2 - 10 % Germany
Natural aggregates 50 - 80 % Germany
Sand 10 - 25 % Germany
Water 2 - 10 % Germany
Technical data
Unit Value
Compressive Strength (Cylinder) N / mm² 35.0
Gross Density kg / m³ 2315.0
Market
Germany
Reference service life
50 years
EPD for the best environmental decision 3
LCA: Calculation rules
Declared unit
1 m³ of WU-Beton C30/37 XC4, XD1, XF1, XM1, XA1; Dmax=32mm
Reference service life
50 years
System boundary
Data quality
The Emidat EPD Tool v1.0.0 was used for LCA modeling and calculation. Background data was used from ecoinvent database
v3.10.
EPD for the best environmental decision 4
System boundaries (X=included, MND=module not declared)
Next product
Production Installation Use stage End-of-Life
system
Module A1 A2 A3 A4 A5 B1 B2 B3 B4 B5 B6 B7 C1 C2 C3 C4 D
Modules
x x x x x x MND MND MND MND MND MND x x x x x
declared
Geography DE DE DE DE MND MND MND MND MND MND DE DE DE DE DE
For the geographies modeled in A1 and A2, refer to Product specification.
Type of EPD: cradle to gate with options, modules C1-C4 and module D (A1-A3, C, D, additional modules A4, A5, and B1)
Stage of Material Production and Construction
Module A1: Extraction and processing of raw materials
Module A2: Transportation of raw materials to the plant
Module A3: Concrete production at the plant and waste treatment
Module A4: Transportation to the construction site
Module A5: Includes processes associated with concrete installation (e.g., pumping on the construction site), as well as the production, transportation, and
treatment of unused concrete
Use Stage
Module B1: Carbonation during the utilization phase
Disposal Stage
Module C1: Demolition/Dismantling
Module C2: Transportation of concrete demolition waste for processing
Module C3: Sorting of waste components and recycling of concrete
Module C4: Disposal of concrete
Credits and burdens outside the system boundaries
Module D: Credits and burdens from the use of demolished concrete as a replacement for primary materials
Cut-off criteria
Environmental impacts of the following processes are considered to be negligible: Production and use of formwork and
falsework for the installation of concrete, Materials used for the curing of concrete (e.g. plastics, aluminum).
Allocation
The allocation is made in accordance with the provisions of EN 15804. Production-process-level elementary flows (energy
and fuels, ancillary materials, and waste) are allocated to the declared unit, using the total production of the production
process for the reference year.
EPD for the best environmental decision 5
ylppus
lairetam
waR
tropsnarT
gnirutcafunaM
tropsnarT
ssecorP
noitallatsnI
esU
ecnanetniaM
riapeR
tnemecalpeR
tnemhsibrufeR
esU
ygrenE
lanoitarepO
esU
retaW
lanoitarepO noitilomeD
tropsnarT
gnissecorP
etsaW
lasopsiD
dnoyeb
sdaol
dna
stfieneB
yradnuob
metsys
eht
LCA: Scenarios and additional technical information
The following information describe the scenarios in the different modules of the EPD.
Transport to the building site (A4) Value Unit
Transported mass 2315.00 kg
Fuel consumption 5.17 L / 100km
Average distance from manufacturer to construction site 13.80 km
Transport mode truck
Gross density of products transported 2315.00 kg / m³
Formwork and Falsework each contribute less than 1% of the total product CO2 emissions, and are therefore neglected
under cut-off rules. (Kaethner, Burridge, 2012). Other sources: Concrete waste: Adams & Hobbs (2023). Electricity, Diesel:
Ecoinvent benchmark average.
Installation into the building (A5) Value Unit
Formwork - kg
Falsework - kg
Concrete waste (installation losses, typical wastage rate on site) 1.50 %
Distance to waste landfill facility (for installation losses) 50 km
Amount of electricity to pour 1 m3 of concrete 3 kWh
Amount of diesel to pour 1 m3 of concrete 60 MJ
Water 0.29 m³
Wastewater treatment 0.29 m³
Calculation of carbonization according to EN 16757. k-factor results from the concrete's compressive strength and its
application. The cement absorption factor (maximum theoretical CO2 uptake) depends on the average clinker content in
cement. The correction factor results from cement substitutes in the recipe.
Use of the installed product (B1) Value Unit
Reference use period 50 years
Building, outside, exposed to
Application
rain
Degree of carbonation (Dc) 0.85 -
Cement absorption factor 0.18 kg CO₂ / kg Cement
k-factor 1.60 mm / year^0.5
Correction factor 1.05 -
Surface area of concrete 5 m²
Specific diesel consumption for a building demolition according to 'Model for Life Cycle Assessment of buildings' (Gervasio,
H. and Dimova, S.). Carbonation during waste processing is not considered. Recycling rate for concrete of 93% reflects the
EPD for the best environmental decision 6
modeled country. Source: Mineralische Bauabfälle Monitoring 2018 Bericht zum Aufkommen und zum Verbleib mineralischer
Bauabfälle im Jahr 2018 (https://kreislaufwirtschaft-bau.de/).
End of life (C1-C4) Value Unit
Material for recycling (total) 2152.95 kg
Distance to waste recycling facility 50 km
Material for landfill (total) 162.05 kg
Distance to waste landfill facility 50 km
Concrete to recycling 2152.95 kg
Diesel required to demolish 1 kg of concrete 0.07 MJ / kg
Calculation of benefits and loads per EN 15804+A2.
Reuse, recovery and/or recycling potentials (D) Value Unit
Amount of recycled material that system takes in 0 kg
Avoided gravel production 2152.95 kg
EPD for the best environmental decision 7
LCA: Results
Core environmental impact indicators
Indicator Unit A1-3 A4 A5 B1 C1 C2 C3 C4 D
GWP-total kg CO₂-eq. 184.53 3.31 10.76 -2.73 16.24 12.00 13.20 1.01 -21.61
GWP-fossil kg CO₂-eq. 184.29 3.31 10.61 -2.73 16.24 11.99 13.20 1.01 -21.56
GWP-biogenic kg CO₂-eq. 0.21 1.7e-03 0.15 0 1.6e-03 6.0e-03 1.3e-03 1.0e-04 -0.02
GWP-luluc kg CO₂-eq. 0.03 1.2e-03 4.0e-03 0 1.4e-03 4.3e-03 1.1e-03 5.3e-04 -0.02
ODP kg CFC-11-Eq 3.6e-06 6.9e-08 1.7e-07 0 2.5e-07 2.5e-07 2.0e-07 2.9e-08 -1.7e-07
AP mol H+-Eq 0.45 7.8e-03 0.07 0 0.15 0.03 0.12 7.2e-03 -0.13
EP-freshwater kg P-Eq 0.04 2.3e-04 2.6e-03 0 4.7e-04 8.4e-04 3.8e-04 8.4e-05 -6.6e-03
EP-marine kg N-Eq 0.04 2.0e-03 0.03 0 0.07 7.4e-03 0.06 2.7e-03 -0.03
EP-terrestrial mol N-Eq 1.25 0.02 0.31 0 0.74 0.08 0.60 0.03 -0.38
POCP kg NMVOC-Eq 0.36 0.01 0.09 0 0.22 0.05 0.18 0.01 -0.10
ADPE kg Sb-Eq 1.6e-04 9.5e-06 8.9e-06 0 5.8e-06 3.4e-05 4.7e-06 1.6e-06 -1.2e-04
ADPF MJ, net calorific value 850.03 49.66 122.05 0 212.36 179.94 172.66 24.85 -258.73
WDP m³ world Eq deprived 66.84 0.25 1.55 0 0.52 0.90 0.42 0.07 -32.26
GWP-total: Global Warming Potential - total GWP-fossil: Global warming potential - fossil GWP-biogenic: Global Warming Potential - biogenic GWP-luluc:
Global Warming Potential - luluc ODP: Depletion potential of the stratospheric ozone layer AP: Acidification potential, Accumulated Exceedance EP-
freshwater: Eutrophication potential - freshwater EP-marine: Eutrophication potential - marine EP-terrestrial: Eutrophication potential - terrestrial POCP:
Photochemical Ozone Creation Potential ADPE: Abiotic depletion potential - non-fossil resources ADPF: Abiotic depletion potential - fossil resources WDP:
Water (user) deprivation potential
The indicated Global Warming Potential (GWP) values are considered gross values. They include impacts from the combustion of waste-derived fuels and
biomass. LCIA data read from ILCD+EPD files are interpreted as gross values.
Net values exclude impacts from the combustion of waste-derived fuels and biomass. For A1-3, net GWP-fossil is 147.39 kg CO₂-eq. , and net GWP-biogenic is
0.21 kg CO₂-eq. .
Additional indicators
Indicator Unit A1-3 A4 A5 B1 C1 C2 C3 C4 D
PM disease incidence 4.1e-06 3.2e-07 1.7e-06 0 4.2e-06 1.2e-06 1.9e-05 1.6e-07 -2.0e-06
IRP kBq U235-Eq 538.22 0.06 8.46 0 0.10 0.22 0.08 0.02 -1.82
ETP-fw CTUe 102.33 11.77 20.19 0 30.09 42.64 24.47 3.40 -117.96
HTP-c CTUh 1.8e-05 2.1e-08 3.0e-07 0 6.3e-08 7.7e-08 5.2e-08 4.6e-09 -2.0e-07
HTP-nc CTUh 1.2e-05 3.3e-08 2.1e-07 0 2.9e-08 1.2e-07 2.3e-08 4.5e-09 -1.8e-07
SQP dimensionless 1050.96 49.95 39.21 0 14.88 180.96 12.10 48.89 -242.19
PM: Potential incidence of disease due to PM emissions IRP: Potential Human exposure efficiency relative to U235 ETP-fw: Potential Comparative Toxic Unit
for ecosystems HTP-c: Potential Comparative Toxic Unit for humans - cancer effects HTP-nc: Potential Comparative Toxic Unit for humans - non-cancer
effects SQP: Potential Soil quality index
IRP: This impact category deals mainly with the eventual impact of low dose ionizing radiation on human health of the nuclear fuel cycle. It does not
consider effects due to possible nuclear accidents, occupational exposure nor due to radioactive waste disposal in underground facilities. Potential ionizing
radiation from the soil, from radon and from some construction materials is also not measured by this indicator.
ETP-fw, HTP-c, HTP-nc and SQP: The results of these environmental impact indicators shall be used with care as the uncertainties on these results are high
or as there is limited experienced with these indicators.
EPD for the best environmental decision 8
Use of resources
Indicator Unit A1-3 A4 A5 B1 C1 C2 C3 C4 D
PERE MJ 151.67 0.79 8.08 0 1.30 2.85 1.06 0.23 -23.45
PERM MJ 0 0 0 0 0 0 0 0 0
PERT MJ 151.67 0.79 8.08 0 1.30 2.85 1.06 0.23 -23.45
PENRE MJ 840.96 49.67 121.92 0 212.36 179.95 172.67 24.85 -258.74
PENRM MJ 9.08 0 0.14 0 0 0 -8.44 0 0
PENRT MJ 850.04 49.67 122.05 0 212.36 179.95 164.22 24.85 -258.74
SM kg 50.00 0 0.75 0 0 0 0 0 2152.95
RSF MJ 0 0 0 0 0 0 0 0 0
NRSF MJ 0 0 0 0 0 0 0 0 0
FW m³ 4.18 7.2e-03 0.08 0 0.01 0.03 0.01 0.03 -0.77
PERE: Primary energy resources - renewable: use as energy carrier PERM: Primary energy resources - renewable: used as raw materials PERT: Primary
energy resources - renewable: total PENRE: Primary energy resources - non-renewable: use as energy carrier PENRM: Primary energy resources - non-
renewable: used as raw materials PENRT: Primary energy resources - non-renewable: total SM: Use of secondary material RSF: Renewable secondary fuels
NRSF: Non-renewable secondary fuels FW: Net use of fresh water
Waste flows
Indicator Unit A1-3 A4 A5 B1 C1 C2 C3 C4 D
HWD kg 0.94 0.07 0.18 0 0.24 0.26 0.19 0.03 -2.02
NHWD kg 30.15 1.45 330.51 0 3.24 5.24 2.64 162.68 -36.07
RWD kg ND 1.5e-05 ND 0 2.3e-05 5.4e-05 1.9e-05 3.9e-06 -4.4e-04
HWD: Hazardous waste disposed NHWD: Non harzardous waste disposed RWD: Radioactive waste disposed
Output flows
Indicator Unit A1-3 A4 A5 B1 C1 C2 C3 C4 D
CRU kg 0 0 0 0 0 0 0 0 0
MFR kg 18.73 0 0.28 0 0 0 2152.95 0 0
MER kg 0 0 0 0 0 0 0 0 0
EEE MJ 0 0 0 0 0 0 0 0 0
EET MJ 0 0 0 0 0 0 0 0 0
CRU: Components for re-use MFR: Materials for recycling MER: Materials for energy recovery EEE: Exported electrical energy EET: Exported thermal energy
Name Value Unit
Biogenic carbon content in product 0 kg C
Biogenic carbon content in accompanying packaging 0 kg C
EPD for the best environmental decision 9
Additional requirements
Greenhouse gas emissions from the use of electricity in the manufacturing phase
GoOs were not used and double quantification is not included.
Electricity Unit Value
Electricity from grid kg CO₂-eq. / kWh 0.47
Additional environmental information
Additional environmental impact indicators required in NPCR Part A for construction products
Indicator Unit A1-3 A4 A5 B1 C1 C2 C3 C4 D
GWP-IOBC kg CO₂-eq. ND 3.31 ND -2.73 16.24 11.99 13.20 1.01 -21.60
GWP-IOBC: Global Warming Potential - Instantaneous oxidation of biogenic carbon
EPD for the best environmental decision 10
Bibliography
DIN EN ISO 14025:2011-10 Environmental labels and declarations - Type III environmental declarations - Principles and procedures
DIN EN ISO 14040:2021-02 Environmental management - Life cycle assessment - Principles and framework
DIN EN ISO 14044:2021-02 Environmental management - Life cycle assessment - Requirements and guidelines
EN 15804:2012+A2:2019 Sustainability of construction works - Environmental product declarations - Core rules for the product
category of construction products
DIN CENTR 15941:2010-11 Sustainability of construction works - Environmental product declarations - Methodology for selection and use
of generic data
DIN EN 15942:2022-04 Sustainability of construction works - Environmental product declarations - Communication format business-
to-business
ISO 21930:2017-07 Sustainability in buildings and civil engineering works - Core rules for environmental product declarations of
construction products and services
Ecoinvent v3.10 ecoinvent, Zurich, Switzerland, database version 3.10
PCR NPCR 020 PART B for concrete and concrete elements (v3.0)
EN 16757 Sustainability of construction works - Environmental product declarations - Product Category Rules for
concrete and concrete elements
Kaethner, S. C. & Burridge, J. A. Embodied CO2 of structural frames. The Structural Engineer 8 (2012)
Adams, K. & Hobbs, G. Final Report: Wastage Rates for Blocks and Ready-Mix Concrete. Reusefully Ltd for MPA (2023):
https://www.aircrete.co.uk/Sustainability-Environmental/Wastage-Rates.aspx
Dos Santos Gervasio, H. and Dimova, S. Environmental benchmarks for buildings , EUR 29145 EN, Publications Office of the European Union, 2018,
ISBN 978-92-79-80969-9 (print),978-92-79-80970-5 (pdf), doi:10.2760/073513 (online),10.2760/90028 (print),
JRC110085.
Basic principles and recommendations for describing the dismantling, post use, and disposal stage of
construction products: https://www.umweltbundesamt.de/sites/default/files/medien/1410/publikationen/2020-07-06_texte_130-2
020_guidance-document-construction-industry.pdf
ILCD Handbook: https://eplca.jrc.ec.europa.eu/uploads/ILCD-Handbook-LCIA-Background-analysis-online-12March2010.pdf
Program Operator Phone +47 23 08 80 00
EPD-Norge
Majorstuen P.O. Box 5250, N-0303 Oslo Email post@epd-norge.no
Norway Web www.epd-norge.no
Publisher Phone +47 23 08 80 00
The Norwegian EPD Foundation
Post Box 5250 Majorstuen, 0303 Oslo Email post@epd-norge.no
Norway Web www.epd-norge.no
Owner of the declaration Phone +49 6131 9179 114
Beyer Baustoffhandelsgesellsch. mbH
Robert-Koch-Str. 32, 55129 Mainz - Hechtsheim Email Oliver.Juli@beyer-
Germany baustoffe.de
Web www.beyer-baustoffe.de
Author of the life cycle assesment Phone +49 6131 9179 114
Beyer Baustoffhandelsgesellsch. mbH
Robert-Koch-Str. 32, 55129 Mainz - Hechtsheim Email Oliver.Juli@beyer-
Germany baustoffe.de
Web www.beyer-baustoffe.de
Web www.eco-platform.org
ECO Platform
ECO Portal
Web ECO Portal
Developer of EPD generator Phone +49 176 56 96 77 91
Emidat GmbH
Sandstraße 33, 80335 München Email epd@emidat.com
Germany Web www.emidat.com
EPD for the best environmental decision 11
