Environmental product declaration
in accordance with ISO 14025 and EN 15804+A2
Sola Universal chair with five star base and height adjustment
Owner of the declaration: Program operator:
Martela Oyj The Norwegian EPD Foundation
Product: Declaration number:
Sola Universal chair with five star base and height
adjustment Registration number:
Declared unit: Issue date:
1 pcs
Valid to:
This declaration is based on Product Category Rules:
EPD Software:
CEN Standard EN 15804:2012+A2:2019 serves as core
The Norwegian EPD Foundation LCA.no EPD generator ID: 61779
PCR
NPCR 026:2022 Part B for Furniture
1 / 13
General information
Product Owner of the declaration:
Sola Universal chair with five star base and height adjustment Martela Oyj
Contact person: Anne-Maria Peitsalo
Phone:
e-mail: anne-maria.peitsalo@martela.com
Program operator: Manufacturer:
Post Box 5250 Majorstuen, 0303 Oslo, Norway Martela Oyj
The Norwegian EPD Foundation Miestentie 1
Phone: +47 23 08 80 00 02150 Espoo, Finland
web: post@epd-norge.no
Declaration number: Place of production:
Martela Oyj, Nummela production
Ojakkalantie 10
03100 Nummela, Finland
This declaration is based on Product Category Rules: Management system:
CEN Standard EN 15804:2012+A2:2019 serves as core PCR ISO 14001, ISO 9001, ISO 45001
NPCR 026:2022 Part B for Furniture
Statement of liability: Organisation no:
The owner of the declaration shall be liable for the underlying 0114891-2
information and evidence. EPD Norway shall not be liable with respect
to manufacturer information, life cycle assessment data and
evidences.​
Declared unit: Issue date:
1 pcs Sola Universal chair with five star base and height adjustment
Declared unit (cradle to gate) with option: Valid to:
A1-A3,A4,A5,B2,B3,B4,C1,C2,C3,C4,D
Year of study:
2022
Functional unit: Comparability:
The Sola chair series include several chair and stool models with EPD of construction products may not be comparable if they not
numerous base options. comply with EN 15804 and seen in a building context.
From the series designed by Antti Kotilainen, it is easy to find a
suitable alternative for different areas of use, such as meeting rooms,
lounges and for office use.
General information on verification of EPD from EPD tools: Development and verification of EPD:
Independent verification of data, other environmental information The declaration is created using EPD tool lca.tools ver EPD2022.03,
and the declaration according to ISO 14025:2010, § 8.1.3 and § 8.1.4. developed by LCA.no. The EPD tool is integrated in the company's
Verification of each EPD is made according to EPD-Norway’s management system, and has been approved by EPD Norway.
guidelines for verification and approval requiring that tools are i)
integrated into the company's environmental management system, ii) Developer of EPD: Tiina Bordi
the procedures for use of the EPD tool are approved by EPD-Norway,
Reviewer of company-specific input data and EPD: Anne-Maria
and iii) the process is reviewed annually by an independent third
Peitsalo
party verifier. See Appendix G of EPD-Norway's General Programme
Instructions for further information on EPD tools
Verification of EPD tool: Approved:
Independent third party verification of the EPD tool, background data
and test-EPD in accordance with EPDNorway's procedures and
guidelines for verification and approval of EPD tools. Håkon Hauan, CEO EPD-Norge
Third party verifier:
Elisabet Amat, GREENIZE projects
(no signature required)
2 / 13
Product
Product description:
Sola universal chair with castors and height adjustment is especially suitable for small meeting rooms and for short term working. The seat height
can be easily adjusted and the tilt mechanism offers additional sitting comfort. The upholstered seat is also available with the more comfy soft
upholstery.
Product specification
Sola universal chair with five star base with no armrests
Fully upholstered seat with Cura/ Gabriel fabric (98% recycled polyester)
Tilt mechanism
Package designed for use of export deliveries (flat-pack)
Recycled share in Recycled share in
Materials kg %
material (kg) material (%)
Metal - Aluminium 1,84 16,31 1,84 100,00
Metal - Steel 4,63 41,05 0,00 0,00
Plastic - Nylon (PA) 0,70 6,21 0,00 0,00
Plastic - Polyurethane (PUR) 1,31 11,62 0,00 0,00
Textile - Polyester (PE) 0,38 3,35 0,37 97,88
Wood - Plywood 2,42 21,46 0,00 0,00
Total 11,28 2,21
Recycled share in Recycled share in
Packaging kg %
material (kg) material (%)
Packaging - Cardboard 1,20 91,60 0,43 36,00
Packaging - Plastic 0,11 8,40 0,00 0,00
Total incl. packaging 12,59 2,64
Technical data:
More product data available:
https://www.martela.com/furniture/seating/universal-chairs/sola-universal-chair-with-five-star-base-and-height-adjustment
Market:
Europe
Reference service life, product
At least 10 years verified by type testing in accredited test laboratory, 5 years warranty
Reference service life, building
LCA: Calculation rules
Declared unit:
1 pcs Sola Universal chair with five star base and height adjustment
Cut-off criteria:
All major raw materials and all the essential energy is included. The production processes for raw materials and energy flows with very small
amounts (less than 1%) are not included. These cut-off criteria do not apply for hazardous materials and substances.
Allocation:
The allocation is made in accordance with the provisions of EN 15804. Incoming energy and water and waste production in-house is allocated
equally among all products through mass allocation. Effects of primary production of recycled materials is allocated to the main product in which
the material was used. The recycling process and transportation of the material is allocated to this analysis.
Data quality:
Specific data for the product composition are provided by the manufacturer. They represent the production of the declared product and were
collected for EPD development in the year of study. Background data is based on registered EPDs according to EN 15804, Ostfold Research
databases, ecoinvent and other LCA databases. The data quality of the raw materials in A1 is presented in the table below.​
3 / 13
Materials Source Data quality Year
Metal - Aluminium ecoinvent 3.6 Database 2019
Metal - Steel ecoinvent 3.6 Database 2019
Packaging - Cardboard ecoinvent 3.6 Database 2019
Packaging - Plastic ecoinvent 3.6 Database 2019
Plastic - Nylon (PA) ecoinvent 3.6 Database 2019
Plastic - Polyurethane (PUR) ecoinvent 3.6 Database 2019
Textile - Polyester (PE) ecoinvent 3.6 Database 2019
Textile - Polyester (PE) Modified ecoinvent 3.6 Database 2019
Wood - Plywood modified ecoinvent 3.6 Database 2019
4 / 13
System boundaries (X=included, MND=module not declared, MNR=module not relevant)
Construction Beyond the system
Product stage Use stage End of life stage
installation stage boundaries
A1 A2 A3 A4 A5 B1 B2 B3 B4 B5 B6 B7 C1 C2 C3 C4 D
X X X X X MND X X X MND MND MND X X X X X
System boundary:
Product Stage / A1 Raw materials:
Martela has long partnerships with its suppliers and subcontractors, who buy raw materials to their products and components from their suppliers,
respectively. Main suppliers are locating in Europe.
Wood material is coming from sustainably cultivated forest (FSC, PEFC, etc) and fabrics can be chosen our standard collection with Öko tex or EU
ecolabel certificates. Recycled materials are taken to use based on availability and when they fulfill the technical requirements set for the end
products.
Materials are including the product package to our customers. Packages that are coming from suppliers are re-used in customer delivery phase
(like pallets) or handled as waste in Manufacturing phase A3. Customer delivery package is disposed in Installation phase A5.
Product Stage / A2 Transport:
Transportation is calculated from suppliers location to our own factories in Nummela, Kitee and Poland and between our factories when delivering
components to final assembly phase in our logistics center in Nummela.
Product Stage / A3 Manufacturing:
Martela has three own factories for manufacturing our products. Kitee factory is manufacturing laminate and melamine components for cabinets
and tables. Poland factory is producing sewing and upholstery parts to chairs and screens. Production unit in Nummela make final assembly of the
products based on customer orders.
Nummela and Kitee factories are using renewable electricity and heating energy. From factory waste 98% is recycled. Poland factory is in rental
premises and cannot choose its used energy, so in calculation we are using Poland average factors.
Additional technical information:
waR slairetam tropsnarT gnirutcafunaM tropsnarT ylbmessA e​sU ecnanetniaM riapeR tnemecalpeR tnemhsibrufeR lanoitarepO ygrene esu lanoitarepO esu retaw -eD noitcurtsnoc noitilomed tropsnarT etsaW gnissecorp lasopsiD -yrevoceR-esueR laitnetop-gnilcyceR
5 / 13
LCA: Scenarios and additional technical information
The following information describe the scenarios in the different modules of the EPD.
Construction installation stage / A4 Transport:
Transportation from Martela logistics center in Nummela to our customers are calculated base on average transportation distances: in Finland 300
km and in Scandinavia 1000 km. In export deliveries Ferry is in use (between Helsinki - Tallinn and Turku - Stockholm).
Construction installation stage / A5 Assembly:
Martela products are partly assembled at customer premises (like tables). This assembling is done with hand tools and use of energy is minimal in
this stage.
Customer end package is disposed in this stage automatically by the tool set-up, but with local installations, our installation personnel take all
waste back to our premises and packages are re-used (like pallets) or recycled locally or in Nummela factory (included in A3 waste).
User stage / B1-B7:
Martela products do not require special maintenance. Cleaning with for example vacuuming and wet wiping is advice according.
Based on technical durability testing according EN standard in accredited testing laboratory Martela verifies use life of at least 10 years and grants
normal warranty for 5 years. Product use life can be extended from that by re-furbishing upholstery parts.
End-of-life stage / C1-C4:
LCA-tool is calculating stage C waste processing and disposal material by material for recycling and resource for energy production in Norway.
Material amounts are calculated based on the material used to make the product.
Beyond the system boundaries / Re-use - Recovery - Recycling -potential / D:
LCA-tool is calculating stage D potential based on material recycling and resource for energy production from materials if product end of lifecycle
would be in Norway. Material amounts are calculated based on the material used to make the product
Capacity utilisation Value
Transport from production place to user (A4) Distance (km) Fuel/Energy Consumption Unit
(incl. return) % (Liter/tonne)
Ship, Ferry, Sea (km) 50,0 % 300 0,034 l/tkm 10,20
Truck, 16-32 tonnes, EURO 6 (km) 36,7 % 800 0,043 l/tkm 34,40
Assembly (A5) Unit Value
Waste, packaging, corrugated board box, to
kg 1,20
average treatment (kg)
Electricity, Nordic (kWh) kWh/DU 0,20
Waste, packaging, plastic film (LDPE), to average
kg 0,11
treatment - A5 (kg)
Maintenance (B2) Unit Value
Electricity, Nordic (kWh) kWh/DU 1,00
Water, tap water (m3) m3/DU 0,00
Capacity utilisation Value
Transport to waste processing (C2) Distance (km) Fuel/Energy Consumption Unit
(incl. return) % (Liter/tonne)
Truck, 16-32 tonnes, EURO 6 (km) 36,7 % 85 0,043 l/tkm 3,66
Waste processing (C3) Unit Value
Waste treatment per kg Plastics, Mixture,
kg 0,70
municipal incineration with fly ash extraction (kg)
Waste treatment per kg Polyurethane (PU),
kg 1,31
incineration (kg)
Waste treatment per kg Scrap aluminium,
kg 1,84
incineration with fly ash extraction (kg)
Waste treatment per kg Scrap steel, incineration
kg 4,63
with fly ash extraction (kg)
Waste treatment per kg Textile, incineration with
kg 0,38
fly ash extraction (kg)
Waste treatment per kg Wood, incineration with
kg 2,42
fly ash extraction (kg)
Waste, materials to recycling (kg) kg 1,76
6 / 13
Disposal (C4) Unit Value
Landfilling of ashes and residues from
kg 1,65
incineration of Scrap aluminium (kg)
Landfilling of ashes and residues from
kg 3,06
incineration of Scrap steel (kg)
Landfilling of ashes from incineration of Plastics,
Mixture, municipal incineration with fly ash
kg 0,02
extraction, process per kg ashes and residues - C4
(kg)
Landfilling of ashes from incineration of
Polyurethane (PU), process per kg ashes and kg 0,05
residues - C4 (kg)
Landfilling of ashes from incineration of Textile,
kg 0,02
soiled, process per kg ashes and residues (kg)
Landfilling of ashes from incineration of Wood,
kg 0,03
process per kg ashes and residues (kg)
Benefits and loads beyond the system
Unit Value
boundaries (D)
Substitution of electricity, in Norway (MJ) MJ 4,94
Substitution of primary steel with net scrap (kg) kg 0,51
Substitution of thermal energy, district heating, in
MJ 74,77
Norway (MJ)
7 / 13
LCA: Results
The LCA results are presented below for the declared unit defined on page 2 of the EPD document.
Environmental impact
Indicator Unit A1-A3 A4 A5 B2 B3
GWP-total kg CO2 -eq 4,71E+01 2,06E+00 2,09E+00 1,46E-01 0
GWP-fossil kg CO2 -eq 5,25E+01 2,06E+00 5,53E-02 1,36E-01 0
GWP-biogenic kg CO2 -eq -5,43E+00 7,88E-04 2,04E+00 2,48E-03 0
GWP-luluc kg CO2 -eq 4,89E-02 8,44E-04 1,49E-03 7,44E-03 0
ODP kg CFC11 -eq 3,39E-06 4,56E-07 7,56E-09 1,47E-08 0
AP mol H+ -eq 2,58E-01 1,83E-02 2,28E-04 6,28E-04 0
EP-FreshWater kg P -eq 2,97E-03 1,47E-05 1,97E-06 9,01E-06 0
EP-Marine kg N -eq 5,08E-02 4,33E-03 6,00E-05 9,92E-05 0
EP-Terrestial mol N -eq 5,33E-01 4,82E-02 6,33E-04 1,33E-03 0
POCP kg NMVOC -eq 1,83E-01 1,38E-02 1,70E-04 3,12E-04 0
ADP-minerals&metals1 kg Sb -eq 8,38E-03 4,82E-05 9,41E-07 2,12E-06 0
ADP-fossil1 MJ 7,15E+02 3,02E+01 1,04E+00 3,67E+00 0
WDP1 m3 3,49E+03 2,51E+01 5,72E+01 2,84E+02 0
Indicator Unit B4 C1 C2 C3 C4 D
GWP-total kg CO2 -eq 0 0 1,75E-01 9,84E+00 5,60E-02 -1,01E+00
GWP-fossil kg CO2 -eq 0 0 1,75E-01 5,25E+00 5,60E-02 -9,96E-01
GWP-biogenic kg CO2 -eq 0 0 7,23E-05 4,59E+00 4,35E-05 -1,21E-03
GWP-luluc kg CO2 -eq 0 0 6,22E-05 4,02E-05 1,64E-05 -1,52E-02
ODP kg CFC11 -eq 0 0 3,96E-08 2,70E-08 1,66E-08 -3,16E-02
AP mol H+ -eq 0 0 5,02E-04 4,16E-03 3,84E-04 -6,37E-03
EP-FreshWater kg P -eq 0 0 1,40E-06 2,85E-06 5,70E-07 -7,32E-05
EP-Marine kg N -eq 0 0 9,94E-05 2,23E-03 1,36E-04 -1,75E-03
EP-Terrestial mol N -eq 0 0 1,11E-03 2,18E-02 1,51E-03 -1,85E-02
POCP kg NMVOC -eq 0 0 4,26E-04 5,24E-03 4,34E-04 -6,30E-03
ADP-minerals&metals1 kg Sb -eq 0 0 4,83E-06 1,14E-06 9,28E-07 -1,40E-05
ADP-fossil1 MJ 0 0 2,64E+00 2,25E+00 1,23E+00 -1,09E+01
WDP1 m3 0 0 2,56E+00 7,54E+00 2,70E+00 -4,80E+01
GWP-total = Global Warming Potential total; GWP-fossil = Global Warming Potential fossil fuels; GWP-biogenic = Global Warming Potential biogenic; GWP-luluc =
Global Warming Potential land use and land use change; ODP = Depletion potential of the stratospheric ozone layer; AP = Acidification potential, Accumulated
Exceedance; EP-freshwater = Eutrophication potential, fraction of nutrients reaching freshwater end compartment: EP-marine = Eutrophication potential, fraction of
nutrients reaching marine end compartment; EP-terrestrial = Eutrophication potential, Accumulated Exceedance; POCP = Formation potential of tropospheric ozone;
ADP-minerals&metals = Abiotic depletion potential for non-fossil resources; ADP-fossil = Abiotic depletion for fossil resources potential; WDP = Water (user)
deprivation potential, deprivation-weighted water consumption
"Reading example: 9,0 E-03 = 9,0*10-3 = 0,009"
*INA Indicator Not Assessed
1. The results of this environmental impact indicator shall be used with care as the uncertainties on these results are high or as there is limited experienced with the
indicator
Remarks to environmental impacts
This product with timeless design is also techically designed to be used for a long time. When you no longer need it someone else can use it. The
product can be refurbished or remanufactured to even extend the service life. Worn-out materials can be recycled or recovered as energy.
8 / 13
Additional environmental impact indicators
Indicator Unit A1-A3 A4 A5 B2 B3
PM Disease incidence 3,52E-06 1,12E-07 2,21E-09 3,34E-09 0
IRP2 kgBq U235 -eq 2,29E+00 1,32E-01 1,81E-02 8,37E-02 0
ETP-fw1 CTUe 1,57E+03 2,15E+01 1,32E+00 4,60E+00 0
HTP-c1 CTUh 1,37E-07 0,00E+00 3,30E-11 1,08E-10 0
HTP-nc1 CTUh 1,10E-06 2,39E-08 1,05E-09 2,84E-09 0
SQP1 dimensionless 8,53E+02 1,81E+01 7,98E-01 2,77E+00 0
Indicator Unit B4 C1 C2 C3 C4 D
PM Disease incidence 0 0 1,07E-08 2,64E-08 6,96E-09 -2,63E-07
IRP2 kgBq U235 -eq 0 0 1,16E-02 4,09E-03 4,97E-03 -3,76E-02
ETP-fw1 CTUe 0 0 1,96E+00 2,41E+01 7,67E-01 -6,51E+01
HTP-c1 CTUh 0 0 0,00E+00 6,64E-10 2,90E-11 -3,33E-09
HTP-nc1 CTUh 0 0 2,14E-09 2,05E-08 7,81E-10 2,65E-08
SQP1 dimensionless 0 0 1,85E+00 3,09E-01 2,71E+00 -4,18E+01
PM = Particulate Matter emissions; IRP = Ionizing radiation – human health; ETP-fw = Eco toxicity – freshwater; HTP-c = Human toxicity – cancer effects; HTP-nc =
Human toxicity – non cancer effects; SQP = Soil Quality (dimensionless)
"Reading example: 9,0 E-03 = 9,0*10-3 = 0,009"
*INA Indicator Not Assessed
1. The results of this environmental impact indicator shall be used with care as the uncertainties on these results are high or as there is limited experienced with the
indicator
2. This impact category deals mainly with the eventual impact of low dose ionizing radiation on human health of the nuclear fuel cycle. It does not consider effects due
to possible nuclear accidents, occupational exposure nor due to radioactive waste disposal in underground facilities. Potential ionizing radiation from the soil, from
radon and from some construction materials is also not measured by this indicator.
9 / 13
Resource use
Indicator Unit A1-A3 A4 A5 B2 B3
PERE MJ 1,65E+02 3,89E-01 7,27E-01 3,61E+00 0
PERM MJ 4,37E+01 0,00E+00 -9,84E+00 0,00E+00 0
PERT MJ 2,09E+02 3,89E-01 -9,11E+00 3,61E+00 0
PENRE MJ 6,36E+02 3,02E+01 1,05E+00 3,73E+00 0
PENRM MJ 8,12E+01 0,00E+00 -4,67E+00 0,00E+00 0
PENRT MJ 7,18E+02 3,02E+01 -3,62E+00 3,73E+00 0
SM kg 2,64E+00 0,00E+00 0,00E+00 0,00E+00 0
RSF MJ 2,00E+00 1,36E-02 7,46E-03 3,65E-02 0
NRSF MJ 1,15E+01 4,55E-02 6,74E-04 6,29E-05 0
FW m3 7,35E-01 2,91E-03 3,43E-03 1,74E-02 0
Indicator Unit B4 C1 C2 C3 C4 D
PERE MJ 0 0 3,78E-02 7,45E-02 2,41E-02 -3,87E+01
PERM MJ 0 0 0,00E+00 -3,39E+01 0,00E+00 0,00E+00
PERT MJ 0 0 3,78E-02 -3,38E+01 2,41E-02 -3,87E+01
PENRE MJ 0 0 2,64E+00 2,25E+00 1,23E+00 -1,09E+01
PENRM MJ 0 0 0,00E+00 -7,65E+01 0,00E+00 0,00E+00
PENRT MJ 0 0 2,64E+00 -7,43E+01 1,23E+00 -1,09E+01
SM kg 0 0 0,00E+00 0,00E+00 0,00E+00 0,00E+00
RSF MJ 0 0 1,35E-03 1,69E-03 6,37E-04 1,36E-02
NRSF MJ 0 0 4,84E-03 0,00E+00 3,83E-02 -1,68E+00
FW m3 0 0 2,83E-04 8,02E-03 1,11E-03 -4,73E-02
PERE = Use of renewable primary energy excluding renewable primary energy resources used as raw materials; PERM = Use of renewable primary energy resources used
as raw materials; PERT = Total use of renewable primary energy resources; PENRE = Use of non renewable primary energy excluding non-renewable primary energy
resources used as raw materials; PENRM = Use of non renewable primary energy resources used as raw materials; PENRT = Total use of non renewable primary energy
resources; SM = Use of secondary materials; RSF = Use of renewable secondary fuels; NRSF = Use of non-renewable secondary fuels; FW = Net use of fresh water
"Reading example: 9,0 E-03 = 9,0*10-3 = 0,009"
*INA Indicator Not Assessed
10 / 13
End of life - Waste
Indicator Unit A1-A3 A4 A5 B2 B3
HWD kg 4,37E-01 1,50E-03 6,88E-05 3,45E-04 0
NHWD kg 1,12E+01 1,22E+00 1,31E+00 2,28E-02 0
RWD kg 2,02E-03 2,06E-04 7,69E-06 3,85E-05 0
Indicator Unit B4 C1 C2 C3 C4 D
HWD kg 0 0 1,36E-04 0,00E+00 4,75E+00 -3,22E-03
NHWD kg 0 0 1,29E-01 0,00E+00 7,27E-02 -3,77E-01
RWD kg 0 0 1,80E-05 0,00E+00 7,58E-06 -3,09E-05
HWD = Hazardous waste disposed; NHWD = Non-hazardous waste disposed; RWD = Radioactive waste disposed
"Reading example: 9,0 E-03 = 9,0*10-3 = 0,009"
*INA Indicator Not Assessed
End of life - Output flow
Indicator Unit A1-A3 A4 A5 B2 B3
CRU kg 0,00E+00 0,00E+00 0,00E+00 0,00E+00 0
MFR kg 1,98E+00 0,00E+00 1,17E+00 0,00E+00 0
MER kg 6,10E-06 0,00E+00 8,39E-02 0,00E+00 0
EEE MJ 7,34E-01 0,00E+00 6,86E-02 0,00E+00 0
EET MJ 1,11E+01 0,00E+00 1,04E+00 0,00E+00 0
Indicator Unit B4 C1 C2 C3 C4 D
CRU kg 0 0 0,00E+00 0,00E+00 0,00E+00 0,00E+00
MFR kg 0 0 0,00E+00 1,76E+00 0,00E+00 0,00E+00
MER kg 0 0 0,00E+00 1,13E+01 0,00E+00 0,00E+00
EEE MJ 0 0 0,00E+00 5,05E+00 0,00E+00 0,00E+00
EET MJ 0 0 0,00E+00 7,64E+01 0,00E+00 0,00E+00
CRU = Components for re-use; MFR = Materials for recycling; MER = Materials for energy recovery; EEE = Exported energy electrical; EET = Exported energy thermal
"Reading example: 9,0 E-03 = 9,0*10-3 = 0,009"
*INA Indicator Not Assessed
Biogenic Carbon Content
Indicator Unit At the factory gate
Biogenic carbon content in product kg C 1,10E+00
Biogenic carbon content in accompanying packaging kg C 5,56E-01
Note: 1 kg biogenic carbon is equivalent to 44/12 kg CO2
11 / 13
Additional requirements
Greenhouse gas emissions from the use of electricity in the manufacturing phase
National production mix from import, low voltage (production of transmission lines, in addition to direct emissions and losses in grid) of applied
electricity for the manufacturing process (A3).
Electricity mix Data source Amount Unit
Electricity, Finland (kWh) ecoinvent 3.6 255,20 g CO2-eq/kWh
Electricity, Poland (kWh) ecoinvent 3.6 1060,47 g CO2-eq/kWh
Dangerous substances
The product contains no substances given by the REACH Candidate list.
Indoor environment
Additional Environmental Information
Key Environmental Indicators
Key environmental indicators Unit A1-A3 A4 A1-C4 A1-D
GWPtotal kg CO2 -eq 47,08 2,06 61,45 60,44
Total energy consumption MJ 815,20 30,63 861,31 810,03
Amount of recycled materials % 20,98
Additional environmental impact indicators required in NPCR Part A for construction products
Indicator Unit A1-A3 A4 A5 B2 B3
GWPIOBC kg CO2 -eq 5,31E+01 2,06E+00 4,82E-02 1,98E-01 0
Indicator Unit B4 C1 C2 C3 C4 D
GWPIOBC kg CO2 -eq 0 0 1,75E-01 5,83E+00 5,94E-02 -1,29E+00
GWP-IOBC: Global warming potential calculated according to the principle of instantaneous oxidation. In order to increase the transparency of biogenic carbon
contribution to climate impact, the indicator GWP-IOBC is required as it declares climate impacts calculated according to the principle of instantaneous oxidation.
GWP-IOBC is also referred to as GWP-GHG in context to Swedish public procurement legislation.
12 / 13
Bibliography
ISO 14025:2010 Environmental labels and declarations - Type III environmental declarations - Principles and procedures.
ISO 14044:2006 Environmental management - Life cycle assessment - Requirements and guidelines.
EN 15804:2012+A2:2019 Environmental product declaration - Core rules for the product category of construction products.
ISO 21930:2017 Sustainability in buildings and civil engineering works - Core rules for environmental product declarations of construction
products.
ecoinvent v3, Allocation, cut-off by classification, Swiss Centre of Life Cycle Inventories.
Iversen et al., (2021) eEPD v2021.09 Background information for EPD generator tool system verification, LCA.no Report number: 07.21
Ruud et al., (2023) EPD generator for NPCR026 Part B for Furniture - Background information for EPD generator application and LCA data,
LCA.no report number 01.23
NPCR Part A: Construction products and services. Ver. 2.0. March 2021, EPD-Norge.
NPCR 026 Part B for Furniture. Ver. 2.0 March 2022, EPD-Norge.
Program operator and publisher Phone: +47 23 08 80 00
The Norwegian EPD Foundation e-mail: post@epd-norge.no
Post Box 5250 Majorstuen, 0303 Oslo, Norway web: www.epd-norge.no
Owner of the declaration: Phone:
anne-
Martela Oyj e-mail:
maria.peitsalo@martela.com
Miestentie 1, 02150 Espoo web: martela.com
Author of the Life Cycle Assessment Phone: +47 916 50 916
LCA.no AS e-mail: post@lca.no
Dokka 6B, 1671 web: www.lca.no
Developer of EPD generator Phone: +47 916 50 916
LCA.no AS e-mail: post@lca.no
Dokka 6B,1671 Kråkerøy web: www.lca.no
ECO Platform web: www.eco-platform.org
ECO Portal web: ECO Portal
13 / 13
