Environmental product declaration
in accordance with ISO 14025 and EN 15804+A2
Isoterm T75-300-600 water 75/125 mm - Isoterm T75-300-600 pressure sewer 75/125
mm
Owner of the declaration: Program operator:
Pipelife Norge AS The Norwegian EPD Foundation
Product: Declaration number:
Isoterm T75-300-600 water 75/125 mm - Isoterm T75-
300-600 pressure sewer 75/125 mm NEPD-8712-8371
Declared unit: Registration number:
1 kg
NEPD-8712-8371
This declaration is based on Product Category Rules:
Issue date: 15.01.2025
CEN Standard EN 15804:2012+A2:2019 serves as core
The Norwegian EPD Foundation PCR Valid to: 15.01.2030
NPCR Part A: Construction products and services. Ver. 2.0
March 2021 EPD software:
LCAno EPD generator ID: 742013
1 / 12
General information
Product Owner of the declaration:
Isoterm T75-300-600 water 75/125 mm - Isoterm T75-300-600 Pipelife Norge AS
pressure sewer 75/125 mm Contact person: Are Lyubråten
Phone: +47 71 65 88 00
e-mail: are.lyubraten@pipelife.com
Program operator: Manufacturer:
The Norwegian EPD Foundation Pipelife Norge AS
Post Box 5250 Majorstuen, 0303 Oslo, Norway Hamnesvegen 97
Phone: +47 977 22 020 6650 Surnadal, Norway
web: www.epd-norge.no
Declaration number: Place of production:
Pipelife Norge AS - Ringebu
NEPD-8712-8371
Flyplassvegen 16
2630 Ringebu, Norway
This declaration is based on Product Category Rules: Management system:
CEN Standard EN 15804:2012+A2:2019 serves as core PCR NS-EN ISO 9001:2015 NS-EN ISO 14001:2015
NPCR Part A: Construction products and services. Ver. 2.0 March
2021
Statement of liability: Organisation no:
The owner of the declaration shall be liable for the underlying 980 457 575
information and evidence. EPD Norway shall not be liable with respect
to manufacturer information, life cycle assessment data and
evidences.​
Declared unit: Issue date:
1 kg Isoterm T75-300-600 water 75/125 mm - Isoterm T75-300-
15.01.2025
600 pressure sewer 75/125 mm
Declared unit (cradle to gate) with option: Valid to:
A1-A3,A4,A5,C1,C2,C3,C4,D 15.01.2030
Year of study:
2022
Functional unit: Comparability:
Not applicable EPD of construction products may not be comparable if they not
comply with EN 15804+A2 and seen in a construction context.
General information on verification of EPD from EPD tools: Development and verification of EPD:
Independent verification of data, other environmental information The declaration is created using EPD tool lca.tools ver EPD2022.03,
and the declaration according to ISO 14025:2010, § 8.1.3 and § 8.1.4. developed by LCA.no. The EPD tool is integrated in the company's
Verification of each EPD is made according to EPD-Norway’s management system, and has been approved by EPD Norway.
guidelines for verification and approval requiring that tools are i) NEPDT15
integrated into the company's environmental management system, ii)
the procedures for use of the EPD tool are approved by EPD-Norway, Developer of EPD: Diana Karin Schleider
and iii) the process is reviewed annually by an independent third
Reviewer of company-specific input data and EPD: Are Lyubråten
party verifier. See Appendix G of EPD-Norway's General Programme
Instructions for further information on EPD tools
Verification of EPD tool: Approved:
Independent third party verification of the EPD tool, background data
and test-EPD in accordance with EPDNorway's procedures and
guidelines for verification and approval of EPD tools.
Third party verifier:
Michael M. Jenssen, Asplan Viak AS
(no signature required)
2 / 12
Product
Product description:
Isoterm pipes water and pressure sewer T75-300-600 are coiled flexible pipes with integrated frost protection. The applications are cold water
supply and sewers under pressure for main and service pipelines to houses, cottages or other facilities, especially when vulnerable landscap,
difficult terrain and cold climates can be a challenge, e.g. during periods when there is a risk of frost.
The pipes have a construction consisting of a media pipe in PE 100 PN16, which is approved for drinking water and a protective corrugated casing
in HDPE, as well as ohmic heating cable as integrated frost protection.
The Isoterm pipes are suitable for permanent installations underground, and in some cases also temporarily for a short period of time above
ground.
More information is found on www.pipelife.no
Product specification
The products covered by this EPD have small variations in composition and are manufactured with the same type of equipment. The composition
below represents an average for these products with components manufactured in 2022.
This EPD presents an average of different configurations within the same dimension of 75/125 mm Isoterm pipe. Within these configurations,
there is a difference in the amounts of cable by weight per DU 1 kg of product.
Variability study has been performed. GWP results A1-A3 between the different configurations deviate between -3% and +2% compared to the
average values presented in this EPD.
Materials kg %
Electronic - Cable 0,04 4,34
Metal - Aluminium 0,00 0,51
Tape 0,00 0,04
Polyethylene (HDPE) 0,89 95,12
Total 0,93 100,00
Packaging kg %
Packaging - Plastic 0,02 29,24
Packaging - Wood 0,05 70,76
Total incl. packaging 1,00 100,00
Technical data:
For products covered by this EPD the following applies:
Media pipes for water supply and sewers fulfill the requirements in accordance with EN 12201 (Nordic Poly Mark). Pipes intended for drinking
water are also approved according to the Danish requirements (DK-VAND).
For technical information, see our handbook:
https://www.pipelife.no/content/dam/pipelife/norway/marketing/general/r%C3%B8rh%C3%A5ndboka/r%C3%B8rh%C3%A5ndboka2021/M-
Materialdata.pdf
Heating cables used as integrated frost protection comply with the requirements of Directive 2014/35/EU (Low Voltage Directive) and are CE-
compliant.
Ohmic heating cables have a nominal power output of 8 W/m (operation mode) and 18 W/m (boost mode).
The circuit lengths range from 15 to 75 m (T75), 60 to 300 m (T300), and 300 to 600 m (T600), based on a 230 VAC supply and C-type
characteristic circuit protection devices in accordance with EN 60898.
Ohmic heating cables are tested and approved according to IEC 60800.
Market:
Mainly Norway, but also the Nordic countries.
Reference service life, product
The overall service lifetime of the assembled product depends on the individual lifetimes of its components and their combined performance.
These lifetimes may vary depending on environmental and operational conditions, compliance with instructions, maintenance, and usage patterns.
Component PE pressure pipe: The service lifetime is at least 100 years. Component heating cable: The expected lifetime is typically 40 to 50 years
for ohmic cables.
Reference service life, building
Not relevant
LCA: Calculation rules
Declared unit:
1 kg Isoterm T75-300-600 water 75/125 mm - Isoterm T75-300-600 pressure sewer 75/125 mm
Cut-off criteria:
All raw materials and all the essential energy are included.
3 / 12
Allocation:
The allocation is made in accordance with the provisions of EN 15804. Incoming energy and waste production in-house is allocated equally among
all products manufactured at Ringebu from raw materials, through mass allocation. The Ringebu factory has its own water supply. Water is not
consumed, it is used for cooling and then returned to natural flows. Effects of primary production of recycled materials is allocated to the main
product in which the material was used. The recycling process and transportation of the material is allocated to this analysis.
Data quality:
Specific data for the product composition are provided by the manufacturer. The data represent the production of the declared product and were
collected for EPD development in the year of study. Background data is based on EPDs according to EN 15804 and different LCA databases. The
data quality of the raw materials in A1 is presented in the table below.
Materials Source Data quality Year
Electronic - Cable ecoinvent 3.6 Database 2019
Metal - Aluminium ecoinvent 3.6 Database 2019
Packaging - Plastic ecoinvent 3.6 Database 2019
Packaging - Wood ecoinvent 3.6 Database 2019
Polyethylene (HDPE) ecoinvent 3.6 Database 2019
Tape ecoinvent 3.6 Database 2019
4 / 12
System boundaries (X=included, MND=module not declared, MNR=module not relevant)
Construction Beyond the system
Product stage Use stage End of life stage
installation stage boundaries
A1 A2 A3 A4 A5 B1 B2 B3 B4 B5 B6 B7 C1 C2 C3 C4 D
X X X X X MND MND MND MND MND MND MND X X X X X
System boundary:
The analysis is a cradle-to-gate (A1 - A3) study, with option A4 transport to market. It includes the extraction and production of raw materials,
transportation to the production site, the production process itself and transport to the market. A5, installation, is included for the transport of
packaging waste from the construction site and the treatment of this waste - not the installation of the products.
Additional technical information:
Professionally executed design, storage, handling, installation, maintenance and operations are a precondition for a long service life. The installation
instructions must be followed.
Pipelife Norway AS is certified according to EN ISO 14001:2015.
See www.pipelife.no for more information on how we are working on environmental issues.
waR slairetam tropsnarT gnirutcafunaM tropsnarT ylbmessA e​sU ecnanetniaM riapeR tnemecalpeR tnemhsibrufeR lanoitarepO ygrene esu lanoitarepO esu retaw -eD noitcurtsnoc noitilomed tropsnarT etsaW gnissecorp lasopsiD -yrevoceR-esueR laitnetop-gnilcyceR
5 / 12
LCA: Scenarios and additional technical information
The following information describe the scenarios in the different modules of the EPD.
Capacity utilisation Value
Transport from production place to user (A4) Distance (km) Fuel/Energy Consumption Unit
(incl. return) % (Liter/tonne)
Truck, 16-32 tonnes, EURO 6 (km) 36,7 % 100 0,043 l/tkm 4,30
Assembly (A5) Unit Value
Waste, hazardous waste, to average treatment
kg 0,00034
(kg)
Waste, packaging, plastic film (LDPE), to average
kg 0,040
treatment - A5 including transport (kg)
Waste, packaging, wood to average treatment -
kg 0,049
A5 including transp. (kg)
Waste processing (C3) Unit Value
Waste treatment of polyethylene (PE),
incineration with energy recovery and fly ash kg 0,47
extraction (kg)
Copper to recycling (kg) kg 0,024
Waste treatment per kg of waste cable, manual
kg 0,040
treatment (kg)
Disposal (C4) Unit Value
Landfilling of ashes from incineration of
Polyethylene (PE), process per kg ashes and kg 0,016
residues (kg)
Landfilling of plastic mixture (kg) kg 0,46
Landfilling of aluminium (kg) kg 0,0047
Waste treatment per kg Copper slag, to landfill,
kg 0,0026
(kg)
Benefits and loads beyond the system
Unit Value
boundaries (D)
Substitution of thermal energy, district heating, in
MJ 14,031
Norway (MJ)
Substitution of electricity, in Norway (MJ) MJ 0,92
6 / 12
LCA: Results
The LCA results are presented below for the declared unit defined on page 2 of the EPD document.
Environmental impact
Indicator Unit A1-A3 A4 A5 C1 C2 C3 C4 D
GWP-total kg CO2 -eq 2,17E+00 1,63E-02 8,10E-02 0 0 1,45E+00 5,41E-02 -8,43E-02
GWP-fossil kg CO2 -eq 2,23E+00 1,63E-02 4,77E-03 0 0 1,45E+00 5,41E-02 -8,13E-02
GWP-biogenic kg CO2 -eq -5,90E-02 6,76E-06 7,62E-02 0 0 2,68E-05 5,25E-06 -1,68E-04
GWP-luluc kg CO2 -eq 2,04E-03 5,81E-06 1,00E-06 0 0 1,13E-05 1,21E-06 -2,80E-03
ODP kg CFC11 -eq 8,65E-08 3,70E-09 4,30E-10 0 0 1,33E-09 1,58E-09 -5,93E-03
AP mol H+ -eq 2,37E-02 4,69E-05 1,52E-05 0 0 2,07E-04 3,99E-05 -6,70E-04
EP-FreshWater kg P -eq 1,64E-04 1,31E-07 2,90E-08 0 0 4,02E-07 6,19E-08 -7,23E-06
EP-Marine kg N -eq 2,19E-03 9,29E-06 8,34E-06 0 0 9,12E-05 6,93E-05 -2,19E-04
EP-Terrestial mol N -eq 2,72E-02 1,04E-04 6,49E-05 0 0 9,89E-04 1,57E-04 -2,37E-03
POCP kg NMVOC -eq 1,02E-02 3,98E-05 1,78E-05 0 0 2,38E-04 5,60E-05 -6,53E-04
ADP-minerals&metals1 kg Sb-eq 1,11E-04 4,51E-07 3,98E-08 0 0 6,69E-08 4,10E-08 -8,09E-07
ADP-fossil1 MJ 6,99E+01 2,47E-01 3,03E-02 0 0 1,63E-01 1,17E-01 -1,16E+00
WDP1 m3 2,04E+02 2,39E-01 7,48E-02 0 0 4,53E-01 1,03E+00 -1,45E+01
GWP-total = Global Warming Potential total; GWP-fossil = Global Warming Potential fossil fuels; GWP-biogenic = Global Warming Potential biogenic; GWP-luluc =
Global Warming Potential land use and land use change; ODP = Depletion potential of the stratospheric ozone layer; AP = Acidification potential, Accumulated
Exceedance; EP-freshwater = Eutrophication potential, fraction of nutrients reaching freshwater end compartment: EP-marine = Eutrophication potential, fraction of
nutrients reaching marine end compartment; EP-terrestrial = Eutrophication potential, Accumulated Exceedance; POCP = Formation potential of tropospheric ozone;
ADP-minerals&metals = Abiotic depletion potential for non-fossil resources; ADP-fossil = Abiotic depletion for fossil resources potential; WDP = Water (user)
deprivation potential, deprivation-weighted water consumption
"Reading example: 9,0 E-03 = 9,0*10-3 = 0,009"
*INA Indicator Not Assessed
1. The results of this environmental impact indicator shall be used with care as the uncertainties on these results are high or as there is limited experienced with the
indicator
Remarks to environmental impacts
Mechanical recycling of PE and heating cables as WEEE is very sustainable and in line with the circular economy. Scrap and used products should
be collected for recycling.
7 / 12
Additional environmental impact indicators
Indicator Unit A1-A3 A4 A5 C1 C2 C3 C4 D
PM Disease incidence 1,06E-07 1,00E-09 2,11E-10 0 0 8,99E-10 7,79E-10 -4,06E-08
IRP2 kgBq U235 -eq 7,20E-02 1,08E-03 1,21E-04 0 0 4,66E-04 5,68E-04 -7,43E-03
ETP-fw1 CTUe 1,67E+02 1,83E-01 3,55E-02 0 0 3,77E-01 3,09E+00 -6,33E+00
HTP-c1 CTUh 2,89E-09 0,00E+00 2,00E-12 0 0 3,30E-11 6,60E-11 -1,16E-10
HTP-nc1 CTUh 1,95E-07 2,00E-10 1,11E-10 0 0 1,26E-09 4,36E-09 -6,07E-09
SQP1 dimensionless 8,62E+00 1,73E-01 3,34E-02 0 0 2,20E-02 4,32E-01 -7,78E+00
PM = Particulate Matter emissions; IRP = Ionizing radiation – human health; ETP-fw = Eco toxicity – freshwater; HTP-c = Human toxicity – cancer effects; HTP-nc =
Human toxicity – non cancer effects; SQP = Soil Quality (dimensionless)
"Reading example: 9,0 E-03 = 9,0*10-3 = 0,009"
*INA Indicator Not Assessed
1. The results of this environmental impact indicator shall be used with care as the uncertainties on these results are high or as there is limited experienced with the
indicator
2. This impact category deals mainly with the eventual impact of low dose ionizing radiation on human health of the nuclear fuel cycle. It does not consider effects due
to possible nuclear accidents, occupational exposure nor due to radioactive waste disposal in underground facilities. Potential ionizing radiation from the soil, from
radon and from some construction materials is also not measured by this indicator.
8 / 12
Resource use
Indicator Unit A1-A3 A4 A5 C1 C2 C3 C4 D
PERE MJ 1,13E+01 3,54E-03 9,59E-04 0 0 1,03E-02 5,65E-03 -7,18E+00
PERM MJ 6,66E-01 0,00E+00 -6,98E-01 0 0 0,00E+00 0,00E+00 0,00E+00
PERT MJ 1,19E+01 3,54E-03 -6,97E-01 0 0 1,03E-02 5,65E-03 -7,18E+00
PENRE MJ 3,36E+01 2,47E-01 3,03E-02 0 0 1,63E-01 1,17E-01 -1,16E+00
PENRM MJ 3,91E+01 0,00E+00 -1,71E+00 0 0 0,00E+00 0,00E+00 0,00E+00
PENRT MJ 7,27E+01 2,47E-01 -1,68E+00 0 0 1,63E-01 1,17E-01 -1,16E+00
SM kg 1,17E-02 0,00E+00 0,00E+00 0 0 0,00E+00 1,65E-07 0,00E+00
RSF MJ 7,40E-02 1,26E-04 2,17E-05 0 0 2,73E-04 1,19E-04 -1,26E-03
NRSF MJ 2,83E-02 4,52E-04 1,67E-04 0 0 0,00E+00 1,88E-03 -4,26E-01
FW m3 9,17E-02 2,64E-05 1,94E-05 0 0 3,04E-04 1,43E-04 -8,65E-03
PERE = Use of renewable primary energy excluding renewable primary energy resources used as raw materials; PERM = Use of renewable primary energy resources used
as raw materials; PERT = Total use of renewable primary energy resources; PENRE = Use of non renewable primary energy excluding non-renewable primary energy
resources used as raw materials; PENRM = Use of non renewable primary energy resources used as raw materials; PENRT = Total use of non renewable primary energy
resources; SM = Use of secondary materials; RSF = Use of renewable secondary fuels; NRSF = Use of non-renewable secondary fuels; FW = Net use of fresh water
"Reading example: 9,0 E-03 = 9,0*10-3 = 0,009"
*INA Indicator Not Assessed
9 / 12
End of life - Waste
Indicator Unit A1-A3 A4 A5 C1 C2 C3 C4 D
HWD kg 1,18E-02 1,27E-05 1,94E-04 0 0 0,00E+00 1,45E-02 -5,47E-05
NHWD kg 2,31E-01 1,20E-02 9,02E-02 0 0 0,00E+00 4,80E-01 -2,75E-02
RWD kg 6,36E-05 1,68E-06 5,80E-09 0 0 0,00E+00 7,69E-07 -6,09E-06
HWD = Hazardous waste disposed; NHWD = Non-hazardous waste disposed; RWD = Radioactive waste disposed
"Reading example: 9,0 E-03 = 9,0*10-3 = 0,009"
*INA Indicator Not Assessed
End of life - Output flow
Indicator Unit A1-A3 A4 A5 C1 C2 C3 C4 D
CRU kg 0,00E+00 0,00E+00 0,00E+00 0 0 0,00E+00 0,00E+00 0,00E+00
MFR kg 7,33E-02 0,00E+00 2,06E-02 0 0 2,40E-02 4,18E-05 0,00E+00
MER kg 2,75E-02 0,00E+00 5,00E-02 0 0 4,78E-01 1,02E-06 0,00E+00
EEE MJ 2,33E-02 0,00E+00 3,47E-02 0 0 9,27E-01 6,61E-05 0,00E+00
EET MJ 3,52E-01 0,00E+00 5,25E-01 0 0 1,40E+01 1,00E-03 0,00E+00
CRU = Components for re-use; MFR = Materials for recycling; MER = Materials for energy recovery; EEE = Exported energy electrical; EET = Exported energy thermal
"Reading example: 9,0 E-03 = 9,0*10-3 = 0,009"
*INA Indicator Not Assessed
Biogenic Carbon Content
Indicator Unit At the factory gate
Biogenic carbon content in product kg C 0,00E+00
Biogenic carbon content in accompanying packaging kg C 1,98E-02
Note: 1 kg biogenic carbon is equivalent to 44/12 kg CO2
10 / 12
Additional requirements
Greenhouse gas emissions from the use of electricity in the manufacturing phase
National production mix from import, low voltage (production of transmission lines, in addition to direct emissions and losses in grid) of applied
electricity for the manufacturing process (A3).
Electricity mix Source Amount Unit
Electricity, Norway (kWh) ecoinvent 3.6 24,33 g CO2-eq/kWh
Dangerous substances
The product contains no substances given by the REACH Candidate list.
Indoor environment
Not relevant
Additional Environmental Information
Additional environmental impact indicators required in NPCR Part A for construction products
Indicator Unit A1-A3 A4 A5 C1 C2 C3 C4 D
GWPIOBC kg CO2 -eq 2,15E+00 1,63E-02 4,73E-03 0 0 1,45E+00 5,41E-02 -8,31E-02
GWP-IOBC: Global warming potential calculated according to the principle of instantaneous oxidation. In order to increase the transparency of biogenic carbon​
contribution to climate impact, the indicator GWP-IOBC is required as it declares climate impacts calculated according to the principle of instantaneous oxidation.​
GWP-IOBC is also referred to as GWP-GHG in context to Swedish public procurement legislation.
11 / 12
Bibliography
ISO 14025:2010 Environmental labels and declarations - Type III environmental declarations - Principles and procedures.
ISO 14044:2006 Environmental management - Life cycle assessment - Requirements and guidelines.
EN 15804:2012+A2:2019 Environmental product declaration - Core rules for the product category of construction products.
ISO 21930:2017 Sustainability in buildings and civil engineering works - Core rules for environmental product declarations of construction
products.
ecoinvent v3, Allocation, cut-off by classification, Swiss Centre of Life Cycle Inventories.
Iversen et al., (2021) eEPD v2021.09 Background information for EPD generator tool system verification, LCA.no rapportnummer: : 07.21.
Vold, et al., (2019) EPD generator for Pipelife - Background information for customer application and LCA data. report number 08.19
NPCR Part A: Construction products and services. Ver. 2.0. March 2021, EPD-Norge.
Program operator and publisher Phone: +47 977 22 020
The Norwegian EPD Foundation e-mail: post@epd-norge.no
Post Box 5250 Majorstuen, 0303 Oslo, Norway web: www.epd-norge.no
Owner of the declaration: Phone: +47 71 65 88 00
Pipelife Norge AS e-mail: are.lyubraten@pipelife.com
Hamnesvegen 97, 6650 Surnadal, Norway web: www.pipelife.no
Author of the Life Cycle Assessment Phone: +47 916 50 916
LCA.no AS e-mail: post@lca.no
Dokka 6A, 1671 Kråkerøy, Norway web: www.lca.no
Developer of EPD generator Phone: +47 916 50 916
LCA.no AS e-mail: post@lca.no
Dokka 6A, 1671 Kråkerøy, Norway web: www.lca.no
ECO Platform web: www.eco-platform.org
ECO Portal web: ECO Portal
12 / 12
