Environmental product declaration
in accordance with ISO 14025 and EN 15804+A2
Leca® ISO 8/20, Leca Norway
Owner of the declaration: Program operator:
Leca International The Norwegian EPD Foundation
Product: Declaration number:
Leca® ISO 8/20, Leca Norway
Registration number:
Declared unit:
1 m3 Issue date:
This declaration is based on Product Category Rules: Valid to:
CEN Standard EN 15804:2012+A2:2019 serves as core
EPD Software:
PCR.
The Norwegian EPD Foundation LCA.no EPD generator ID: 55341
NPCR 012:2018 Part B for Thermal insulation products
1 / 11
General information
Product Owner of the declaration:
Leca® ISO 8/20, Leca Norway Leca International
Contact person: Tone Storbråten
Phone: +47 41 43 71 00
e-mail: info@leca.no
Program operator: Manufacturer:
Post Box 5250 Majorstuen, 0303 Oslo, Norway Leca International
The Norwegian EPD Foundation Årnesvegen 1
Phone: +47 23 08 80 00 2009 Nordby, Norway
web: post@epd-norge.no
Declaration number: Place of production:
Leca, Rælingen
Årnesvegen 1
N-2009 Nordby, Norway
This declaration is based on Product Category Rules: Management system:
CEN Standard EN 15804:2012+A2:2019 serves as core PCR. ISO 14001ISO 9001
NPCR 012:2018 Part B for Thermal insulation products
Statement of liability: Organisation no:
The owner of the declaration shall be liable for the underlying 918 799 141
information and evidence. EPD Norway shall not be liable with respect
to manufacturer information, life cycle assessment data and
evidences.​
Declared unit: Issue date:
1 m3 Leca® ISO 8/20, Leca Norway
Declared unit with option: Valid to:
A1,A2,A3,A4,A5,C1,C2,C3,C4,D
Year of study:
2021
Functional unit: Comparability:
EPD of construction products may not be comparable if they not
comply with EN 15804:2012+A2:2019 and seen in a building context.
General information on verification of EPD from EPD tools: Development and verification of EPD:
Independent verification of data, other environmental information The declaration is created using EPD tool lca.tools ver EPD2022.03,
and the declaration according to ISO 14025:2010, § 8.1.3 and § 8.1.4. developed by LCA.no. The EPD tool is integrated in the company's
Verification of each EPD is made according to EPD-Norway’s management system, and has been approved by EPD Norway.
guidelines for verification and approval requiring that tools are i)
integrated into the company's environmental management system, ii) Developer of EPD: Ana Raquel Fernandes
the procedures for use of the EPD tool are approved by EPD-Norway,
Reviewer of company-specific input data and EPD:​ Tone Storbråten
and iii) the process is reviewed annually by an independent third
party verifier. See Appendix G of EPD-Norway's General Programme
Instructions for further information on EPD tools
Verification of EPD tool: Approved:
Independent third party verification of the EPD tool, background data
and test-EPD in accordance with EPDNorway's procedures and
guidelines for verification and approval of EPD tools.
Third party verifier:
Elisabet Amat - GREENIZE projects
(no signature required)
2 / 11
Product
Product description:
Leca® ISO 8/20 lightweight expanded clay aggregate (LWA) is a porous, ceramic material made from natural clay. Organic matter is mixed into
raw clay, which is pelletized, dried and heated in a rotary kiln at about 1150 °C. The process expands the material into granules with 5x times the
volume of the original clay. The unsorted output material is sieved and blended into different grades of products, followed by distribution in big
bags or as bulk. Leca® ISO 8/20 has a grading of 8/20 mm, a dry bulk density of 245 kg/m³ and have been treated to give the material water
repellent properties to minimize capillary suction.
Product specification
This EPD describes the performance for the production of Leca® ISO 8/20 lightweight expanded clay aggregate, grading 8/20 mm, produced at
Leca Rælingen in Norway. The grading vs. densities list stated in the technical data section can be used for calculations of the environmental
impact of other gradings than 8/20 mm.
Intended use: Leca® ISO 8/20 is intended to be used as thermal insulation layer, drainage material and weight-reducing backfill for infrastructure.
The material is suited in road and railroad embankments, as well and other geotechnical applications, e.g. for earth pressure reduction on retaining
walls. Leca® ISO 8/20 can be used in local water management solutions for handling of stormwater and climate adaptation purposes. Leca® ISO
8/20 is treated with coating to give the surface water repellent properties to minimize capillary suction.
Materials Value Unit
Clay 98,3 %
Waste raw materials 0,2 %
Dolomite 1,5 %
Technical data:
Characteristic values for Leca® ISO 8/20: For additional information, visit www.leca.no
Loose bulk density (NS-EN 1097-3): 245 kg/m³
Grading (NS-EN 933-1): 8/20 mm
Compressive strength, 10% (NS-EN 13055-1): 0,8 MPa
Compressive strength, 2% (NS-EN 13055-1): 0,3 MPa
Thermal conductivity (NS-EN 14063-1), dry: 0,104 W/mK
Reaction to fire (NS-EN 13820): Eurocode A1
Resistance to dynamic loads (NS-EN 15732): < 1,0 % (120 kPa, 2 000 000 cycles)
Market:
Norway
Reference service life, product
Not relevant.
Reference service life, building or construction works
Not relevant.
LCA: Calculation rules
Declared unit:
1 m3 Leca® ISO 8/20, Leca Norway
Cut-off criteria:
All major raw materials and all the essential energy is included. The production processes for raw materials and energy flows with very small
amounts (less than 1%) are not included. These cut-off criteria do not apply for hazardous materials and substances.
Allocation:
The allocation is made in accordance with the provisions of EN 15804+A2. Incoming energy and water and waste production in-house is allocated
equally among all products through mass allocation. Effects of primary production of recycled materials is allocated to the main product in which
the material was used. The recycling process and transportation of the material is allocated to this analysis.
Data quality:
Specific data for the product composition are provided by the manufacturer. The data represent the production of the declared product and were
collected for EPD development in the year of study. Background data is based on EPDs according to EN 15804 and different LCA databases. The
data quality of the raw materials in A1 is presented in the table below.
Materials Source Data quality Year
Additives ecoinvent 3.6 Database 2019
Coating materials ecoinvent 3.6 Database 2019
Dolomite ecoinvent 3.6 Database 2019
Oxygen ecoinvent 3.6 Database 2019
Clay LCA.no Database 2021
3 / 11
System boundaries (X=included, MND=module not declared, MNR=module not relevant)
Construction Beyond the system
Product stage Use stage End of life stage
installation stage boundaries
A1 A2 A3 A4 A5 B1 B2 B3 B4 B5 B6 B7 C1 C2 C3 C4 D
X X X X X MND MND MND MND MND MND MND X X X X X
System boundary:
Additional technical information:
Leca® ISO 8/20 is resistant to degradation, frost and high temperatures. The compound is ceramic and chemically inert.
waR slairetam tropsnarT gnirutcafunaM tropsnarT ylbmessA e​sU ecnanetniaM riapeR tnemecalpeR tnemhsibrufeR lanoitarepO ygrene esu lanoitarepO esu retaw -eD noitcurtsnoc noitilomed tropsnarT etsaW gnissecorp lasopsiD -yrevoceR-esueR laitnetop-gnilcyceR
4 / 11
LCA: Scenarios and additional technical information
The following information describe the scenarios in the different modules of the EPD.
The material has an indefinite service life and require no maintenance during its utilization. Leca® ISO 8/20 can be excavated and re-used in
fillings in other construction projects.
Transport from production site to user (A4): Assuming 50 km transportation distance with a full size truck to the construction site. The weight of
Leca® ISO 8/20 is low, and the loading capacity is therefore limited by the maximum transportation volume of the truck, not its weight capacity.
Capacity utilisation Value
Transport from production place to user (A4) Distance (km) Fuel/Energy Consumption Unit
(incl. return) % (Liter/tonne)
Truck, over 32 tonnes, EURO 6 (km) 53,3 % 50 0,023 l/tkm 1,15
Assembly (A5) Unit Value
Blowing, Machine operation, diesel, > 18.64 kW
h/DU 0,03
(per hour)
Bulldozer, Machine operation, diesel, >=74.57 kW
h/DU 0,02
(per hour)
Crane, Machine operation, diesel, >=74.57 kW
h/DU 0,01
(per hour)
Vibrating plate (per liter diesel) L/DU 0,01
De-construction demolition (C1) Unit Value
Removal of LWA, Machine operation, diesel, >=
h/DU 0,04
74.57 kW (per hour)
Sorting per kg of LWA, for waste treatment after
kg/DU 245,00
removal (kg)
Capacity utilisation Value
Transport to waste processing (C2) Distance (km) Fuel/Energy Consumption Unit
(incl. return) % (Liter/tonne)
Truck, 16-32 tonnes, EURO 5 (km) 36,7 % 50 0,044 l/tkm 2,20
Waste processing (C3) Unit Value
Waste treatment, reuse of LWA (kg) kg 183,75
Disposal (C4) Unit Value
Disposal, landfilling of waste LWA (kg) kg 61,25
Benefits and loads beyond the system
Unit Value
boundaries (D)
Substitution of primary expanded clay (kg) kg 183,75
5 / 11
LCA: Results
The LCA results are presented below for the declared unit defined on page 2 of the EPD document.
Environmental impact
Indicator Unit A1 A2 A3 A4 A5 C1 C2 C3 C4 D
GWP-total
kg CO2 -
1,88E+00 5,51E-01 4,95E+01 1,07E+00 1,27E+00 8,67E-01 2,04E+00 0,00E+00 5,03E-01 -4,62E+01
eq
GWP-fossil
kg CO2 -
2,64E+00 5,50E-01 4,95E+01 1,07E+00 1,27E+00 8,67E-01 2,04E+00 0,00E+00 5,02E-01 -4,60E+01
eq
GWP-biogenic
kg CO2 -
-2,02E+00 2,27E-04 3,46E-03 4,57E-04 2,39E-04 1,61E-04 8,33E-04 0,00E+00 5,87E-04 -1,13E-01
eq
GWP-luluc
kg CO2 -
1,27E+00 1,61E-04 3,26E-03 3,25E-04 9,96E-05 6,79E-05 7,14E-04 0,00E+00 1,23E-04 -1,80E-02
eq
kg
ODP CFC11 - 3,52E-07 1,28E-07 3,77E-07 2,57E-07 2,73E-07 1,86E-07 4,66E-07 0,00E+00 1,90E-07 -2,71E-06
eq
mol H+
AP 2,58E-02 2,26E-03 2,05E-01 3,44E-03 5,70E-03 3,16E-03 8,35E-03 0,00E+00 4,47E-03 -3,67E-01
-eq
EP-FreshWater kg P -eq 2,55E-04 4,21E-06 2,87E-03 8,49E-06 4,60E-06 3,13E-06 1,60E-05 0,00E+00 5,69E-06 -2,29E-03
EP-Marine kg N -eq 1,41E-02 6,67E-04 9,28E-02 7,52E-04 2,09E-03 1,05E-03 2,48E-03 0,00E+00 1,66E-03 -4,59E-02
mol N -
EP-Terrestial 8,22E-02 7,38E-03 1,03E+00 8,39E-03 2,31E-02 1,16E-02 2,74E-02 0,00E+00 1,83E-02 -5,53E-01
eq
kg
POCP NMVOC 1,26E-02 2,40E-03 2,63E-01 3,29E-03 6,70E-03 3,56E-03 8,38E-03 0,00E+00 5,25E-03 -1,49E-01
-eq
ADP- kg Sb -
8,13E-05 9,44E-06 9,69E-06 1,90E-05 1,94E-06 1,32E-06 5,53E-05 0,00E+00 4,53E-06 -6,09E-04
minerals&metals1 eq
ADP-fossil1 MJ 4,79E+01 8,59E+00 3,69E+02 1,73E+01 1,74E+01 1,18E+01 3,08E+01 0,00E+00 1,38E+01 -4,67E+02
WDP1 m3 1,27E+03 6,59E+00 -3,65E+02 1,33E+01 3,70E+00 2,52E+00 2,94E+01 0,00E+00 8,53E+01 -8,63E+02
GWP-total = Global Warming Potential total; GWP-fossil = Global Warming Potential fossil fuels; GWP-biogenic = Global Warming Potential biogenic; GWP-luluc =
Global Warming Potential land use and land use change; ODP = Depletion potential of the stratospheric ozone layer; AP = Acidification potential, Accumulated
Exceedance; EP-freshwater = Eutrophication potential, fraction of nutrients reaching freshwater end compartment: EP-marine = Eutrophication potential, fraction of
nutrients reaching marine end compartment; EP-terrestrial = Eutrophication potential, Accumulated Exceedance; POCP = Formation potential of tropospheric ozone;
ADP-minerals&metals = Abiotic depletion potential for non-fossil resources; ADP-fossil = Abiotic depletion for fossil resources potential; WDP = Water (user)
deprivation potential, deprivation-weighted water consumption
"Reading example: 9,0 E-03 = 9,0*10-3 = 0,009"
*INA Indicator Not Assessed
1. The results of this environmental impact indicator shall be used with care as the uncertainties on these results are high or as there is limited experienced with the
indicator
Remarks to environmental impacts
The clay is excavated from a local clay fields that are close to the factories. Consequently, the production transportation (A2) emissions and costs
are minimized. After depletion all clay fields are remediated back into their original state, e.g. farmlands or natural areas.
Due to polluter-pay-principle, the emissions from waste are not included.
Biogenic carbon from biofuels are balanced to zero since they have their input and output in the same module.
6 / 11
Additional environmental impact indicators
Indicator Unit A1 A2 A3 A4 A5 C1 C2 C3 C4 D
PM Disease incidence 2,47E-07 4,86E-08 1,04E-06 9,80E-08 9,99E-08 6,20E-08 1,47E-07 0,00E+00 9,54E-08 -3,42E-06
IRP2 kgBq U235 -eq 3,53E-01 3,76E-02 1,95E-01 7,57E-02 7,45E-02 5,08E-02 1,35E-01 0,00E+00 6,31E-02 -9,68E-01
ETP-fw1 CTUe 1,02E+02 6,29E+00 5,97E+02 1,27E+01 9,52E+00 6,48E+00 2,27E+01 0,00E+00 7,54E+00 -1,13E+03
HTP-c1 CTUh 7,11E-09 0,00E+00 1,11E-09 0,00E+00 1,08E-09 7,22E-10 0,00E+00 0,00E+00 3,06E-10 -2,06E-08
HTP-nc1 CTUh 9,66E-08 6,08E-09 3,32E-08 1,23E-08 8,04E-09 5,15E-09 2,45E-08 0,00E+00 5,45E-09 -5,57E-07
SQP1 dimensionless 6,79E+01 9,86E+00 3,92E+01 1,99E+01 2,21E+00 1,50E+00 2,12E+01 0,00E+00 5,32E+01 -6,50E+02
PM = Particulate Matter emissions; IRP = Ionizing radiation – human health; ETP-fw = Eco toxicity – freshwater; HTP-c = Human toxicity – cancer effects; HTP-nc =
Human toxicity – non cancer effects; SQP = Potential Soil Quality Index (dimensionless)
"Reading example: 9,0 E-03 = 9,0*10-3 = 0,009"
*INA Indicator Not Assessed
1. The results of this environmental impact indicator shall be used with care as the uncertainties on these results are high or as there is limited experienced with the
indicator
2. This impact category deals mainly with the eventual impact of low dose ionizing radiation on human health of the nuclear fuel cycle. It does not consider effects due
to possible nuclear accidents, occupational exposure nor due to radioactive waste disposal in underground facilities. Potential ionizing radiation from the soil, from
radon and from some construction materials is also not measured by this indicator.
7 / 11
Resource use
Indicator Unit A1 A2 A3 A4 A5 C1 C2 C3 C4 D
PERE MJ 2,81E+01 1,08E-01 5,61E+01 2,18E-01 9,41E-02 6,41E-02 4,35E-01 0,00E+00 4,95E-01 -1,26E+02
PERM MJ 0,00E+00 0,00E+00 0,00E+00 0,00E+00 0,00E+00 0,00E+00 0,00E+00 0,00E+00 0,00E+00 0,00E+00
PERT MJ 2,81E+01 1,08E-01 5,61E+01 2,18E-01 9,41E-02 6,41E-02 4,35E-01 0,00E+00 4,95E-01 -1,26E+02
PENRE MJ 5,22E+01 8,60E+00 3,69E+02 1,73E+01 1,74E+01 1,18E+01 3,08E+01 0,00E+00 1,38E+01 -4,67E+02
PENRM MJ 0,00E+00 0,00E+00 0,00E+00 0,00E+00 0,00E+00 0,00E+00 0,00E+00 0,00E+00 0,00E+00 0,00E+00
PENRT MJ 5,22E+01 8,60E+00 3,69E+02 1,73E+01 1,74E+01 1,18E+01 3,08E+01 0,00E+00 1,38E+01 -4,67E+02
SM kg 6,35E-01 0,00E+00 2,35E-02 0,00E+00 8,54E-03 5,82E-03 0,00E+00 0,00E+00 6,00E-03 -6,90E-01
RSF MJ 4,12E-01 3,78E-03 6,36E-03 7,63E-03 2,32E-03 1,58E-03 1,56E-02 0,00E+00 1,03E-02 -3,34E+00
NRSF MJ 7,73E-02 1,27E-02 4,22E+02 2,56E-02 3,41E-02 2,32E-02 5,55E-02 0,00E+00 2,22E-02 -2,61E+00
FW m3 1,89E-01 9,79E-04 4,07E-02 1,97E-03 8,95E-04 6,10E-04 3,24E-03 0,00E+00 1,70E-02 -3,10E-01
PERE = Use of renewable primary energy excluding renewable primary energy resources used as raw materials; PERM = Use of renewable primary energy resources used
as raw materials; PERT = Total use of renewable primary energy resources; PENRE = Use of non renewable primary energy excluding non-renewable primary energy
resources used as raw materials; PENRM = Use of non renewable primary energy resources used as raw materials; PENRT = Total use of non renewable primary energy
resources; SM = Use of secondary materials; RSF = Use of renewable secondary fuels; NRSF = Use of non-renewable secondary fuels; FW = Net use of fresh water
"Reading example: 9,0 E-03 = 9,0*10-3 = 0,009"
*INA Indicator Not Assessed
8 / 11
End of life - Waste
Indicator Unit A1 A2 A3 A4 A5 C1 C2 C3 C4 D
HWD kg 2,14E-02 4,70E-04 1,14E-02 9,48E-04 5,12E-04 3,49E-04 1,57E-03 0,00E+00 9,74E-04 -5,14E-02
NHWD kg 4,24E-01 7,48E-01 3,06E-01 1,51E+00 2,06E-02 1,40E-02 1,47E+00 0,00E+00 6,13E+01 -3,24E+00
RWD kg 2,68E-04 5,87E-05 1,85E-04 1,18E-04 1,21E-04 8,22E-05 2,10E-04 0,00E+00 9,00E-05 -1,39E-03
HWD = Hazardous waste disposed; NHWD = Non-hazardous waste disposed; RWD = Radioactive waste disposed
"Reading example: 9,0 E-03 = 9,0*10-3 = 0,009"
*INA Indicator Not Assessed
End of life - Output flow
Indicator Unit A1 A2 A3 A4 A5 C1 C2 C3 C4 D
CRU kg 0,00E+00 0,00E+00 0,00E+00 0,00E+00 0,00E+00 0,00E+00 0,00E+00 0,00E+00 0,00E+00 0,00E+00
MFR kg 3,53E-02 0,00E+00 4,80E-02 0,00E+00 8,26E-03 5,71E-03 0,00E+00 1,84E+02 5,47E-03 -5,60E-01
MER kg 5,27E-01 0,00E+00 7,84E-04 0,00E+00 1,55E-04 1,77E-05 0,00E+00 0,00E+00 1,03E-04 -3,35E-02
EEE MJ 1,62E-02 0,00E+00 2,00E-02 0,00E+00 8,92E-05 6,07E-05 0,00E+00 0,00E+00 8,50E-03 -7,30E-02
EET MJ 2,44E-01 0,00E+00 3,02E-01 0,00E+00 1,35E-03 9,19E-04 0,00E+00 0,00E+00 1,29E-01 -1,10E+00
CRU = Components for re-use; MFR = Materials for recycling; MER = Materials for energy recovery; EEE = Exported energy electrical; EET = Exported energy thermal
"Reading example: 9,0 E-03 = 9,0*10-3 = 0,009"
*INA Indicator Not Assessed
Biogenic Carbon Content
Indicator Unit At the factory gate
Biogenic carbon content in product kg C 0,00E+00
Biogenic carbon content in accompanying packaging kg C 0,00E+00
Note: 1 kg biogenic carbon is equivalent to 44/12 kg CO2
9 / 11
Additional requirements
Greenhouse gas emissions from the use of electricity in the manufacturing phase
National production mix from import, low voltage (production of transmission lines, in addition to direct emissions and losses in grid) of applied
electricity for the manufacturing process (A3).
Electricity mix Data source Amount Unit
Renewable electricity Saint-Gobain, based on 100% hydro power, with Guarantee of Origin from LOS 2021 (kWh) ecoinvent 3.6 4,26 g CO2-eq/kWh
Dangerous substances
The product contains no substances given by the REACH Candidate list or the Norwegian priority list.
Indoor environment
Not relevant, see intended uses.
Additional Environmental Information
Additional environmental impact indicators required in NPCR Part A for construction products
Indicator Unit A1 A2 A3 A4 A5 C1 C2 C3 C4 D
GWPIOBC kg CO2 -eq 4,12E+00 5,51E-01 5,85E+00 1,07E+00 1,99E-01 1,98E-01 2,04E+00 0,00E+00 0,00E+00 -4,61E+01
GWP-IOBC: Global warming potential calculated according to the principle of instantaneous oxidation. In order to increase the transparency of biogenic carbon​
contribution to climate impact, the indicator GWP-IOBC is required as it declares climate impacts calculated according to the principle of instantaneous oxidation.​
GWP-IOBC is also referred to as GWP-GHG in context to Swedish public procurement legislation.
10 / 11
Bibliography
ISO 14025:2010 Environmental labels and declarations - Type III environmental declarations - Principles and procedures.
ISO 14044:2006 Environmental management - Life cycle assessment - Requirements and guidelines.
EN 15804:2012+A2:2019 Environmental product declaration - Core rules for the product category of construction products.
ISO 21930:2017 Sustainability in buildings and civil engineering works - Core rules for environmental product declarations of construction
products.
ecoinvent v3, Allocation, cut-off by classification, Swiss Centre of Life Cycle Inventories.
Iversen et al., (2021) eEPD v2021.09 Background information for EPD generator tool system verification, LCA.no Report number: 07.21
Vold et. al., (2022) EPD generator for NPCR 012 Thermal insulation, Background information for EPD generator application and LCA data, LCA.no
report number: 07.22.
NPCR Part A: Construction products and services. Ver. 2.0. April 2021, EPD-Norge.
NPCR 012 Part B for Part B for Thermal insulation products, Ver. 2.0, 31.03.2022, EPD Norway.
Program operator and publisher Phone: +47 23 08 80 00
The Norwegian EPD Foundation e-mail: post@epd-norge.no
Post Box 5250 Majorstuen, 0303 Oslo, Norway web: www.epd-norge.no
Owner of the declaration: Phone: +47 41 43 71 00
Leca International e-mail: info@leca.no
Årnesvegen 1, 2009 Nordby web: www.leca.no
Author of the Life Cycle Assessment Phone: +47 916 50 916
LCA.no AS e-mail: post@lca.no
Dokka 6B, 1671 web: www.lca.no
Developer of EPD generator Phone: +47 916 50 916
LCA.no AS e-mail: post@lca.no
Dokka 6B,1671 Kråkerøy web: www.lca.no
ECO Platform web: www.eco-platform.org
ECO Portal web: ECO Portal
11 / 11
