Environmental product declaration
in accordance with ISO 14025 and EN 15804+A2
LAPP ÖLFLEX® CLASSIC 115 CY 4X0,5 BK Elnr 1025648
Owner of the declaration: Program operator:
Lapp Norway AS The Norwegian EPD Foundation
Product: Declaration number:
LAPP ÖLFLEX® CLASSIC 115 CY 4X0,5 BK Elnr 1025648 NEPD-9232-8809
Declared unit: Registration number:
1 m NEPD-9232-8809
This declaration is based on Product Category Rules: Issue date:
CEN Standard EN 15804:2012+A2:2019 serves as core 24.02.2025
PCR
Valid to:
The Norwegian EPD Foundation NPCR 027:2020 Part B for Electrical cables and wires
24.02.2030
EPD software:
LCAno EPD generator ID: 765673
1 / 12
General information
Product Owner of the declaration:
LAPP ÖLFLEX® CLASSIC 115 CY 4X0,5 BK Elnr 1025648 Lapp Norway AS
Contact person: Petter Dahl
Phone: 91597046
e-mail: petter.dahl@lapp.com
Program operator: Manufacturer:
The Norwegian EPD Foundation Lapp Norway AS
Post Box 5250 Majorstuen, 0303 Oslo, Norway Eikringen 11
Phone: +47 977 22 020 3036 Drammen, Norway
web: www.epd-norge.no
Declaration number: Place of production:
Cableries Lapp S.a.r.l.
NEPD-9232-8809
Technopole Sud Forbach
F - 57600 FORBACH, France
This declaration is based on Product Category Rules: Management system:
CEN Standard EN 15804:2012+A2:2019 serves as core PCR ISO 14001, ISO 9001
NPCR 027:2020 Part B for Electrical cables and wires
Statement of liability: Organisation no:
The owner of the declaration shall be liable for the underlying 919 398 876
information and evidence. EPD Norway shall not be liable with respect
to manufacturer information, life cycle assessment data and
evidences.​
Declared unit: Issue date:
1 m LAPP ÖLFLEX® CLASSIC 115 CY 4X0,5 BK Elnr 1025648 24.02.2025
Declared unit with option: Valid to:
A1,A2,A3,A4,A5,B6,C1,C2,C3,C4,D 24.02.2030
Year of study:
2023
Functional unit: Comparability:
1 meter of ÖLFLEX® CLASSIC 115 CY 4X0,5 BK mm2 from cradle-to- EPD of construction products may not be comparable if they not
grave. comply with EN 15804 and seen in a building context.
General information on verification of EPD from EPD tools: Development and verification of EPD:
Independent verification of data, other environmental information The declaration is created using EPD tool lca.tools ver EPD2022.03,
and the declaration according to ISO 14025:2010, § 8.1.3 and § 8.1.4. developed by LCA.no. The EPD tool is integrated in the company's
Verification of each EPD is made according to EPD-Norway’s management system, and has been approved by EPD Norway.
guidelines for verification and approval requiring that tools are i) Approval number: NEPDT133
integrated into the company's environmental management system, ii)
the procedures for use of the EPD tool are approved by EPD-Norway, Developer of EPD: Julie Olsson
and iii) the process is reviewed annually by an independent third
Reviewer of company-specific input data and EPD:​ Lars Nilsen
party verifier. See Appendix G of EPD-Norway's General Programme
Instructions for further information on EPD tools
Verification of EPD tool: Approved:
Independent third party verification of the EPD tool, background data
and test-EPD in accordance with EPDNorway's procedures and
guidelines for verification and approval of EPD tools. Approval
number: NEPDT32.
Third party verifier:
Vito D’Incognito, Take Care International
(no signature required)
2 / 12
Product
Product description:
Application
ÖLFLEX CLASSIC 115 CY cables are control cables for occasional flexible use and fixed installation under medium mechanical load
conditions. They are also suitable for use in dry, damp or wet areas. If using outdoors, observe the indicated temperature range, They are largely
resistant to acids, alkalis and certain oils at room temperature.
ÖLFLEX CLASSIC 115 CY cables are suitable for occasional, non-automated movements. They meet the requirements for slow rotational
movements, such as in the loop of a wind turbine. The maximum tensile load is 15 N/mm² of conductor cross-section during installation and
operation. Compulsory guidance is not permitted.
The screening braid protects against interference from electrical fields.
Application range:
Control units for machine tools, conveyor systems, measurement and control technology, office machines and systems for data processing.
This cable is suitable for torsion application in wind turbines (WTG). The torsional load is limited to applications, as they typically occur in the
loop of a wind turbine.
Product specification
Design
Design based on EN 50525-2-51
Certification EN 13501-6 and EN 50575
Classification of fire behaviour
(article/dimension range see www.lappkabel.com/cpr)
Conductor fine wire strands of bare copper acc. to IEC 60228 resp. EN 60228, class 5
Insulation PVC compound TI2 acc. to EN 50363-3
with increased requirements acc. to Lapp specification
Core identification code acc. to VDE 0293-1, with or without GN/YE ground conductor
black cores with white numbers acc. to EN 50334
Stranding cores are stranded in layers
Wrapping plastic foil
Screen braid of tinned copper, coverage = 85 % (nominal value)
Outer sheath PVC compound TM2 acc. to EN 50363-4-1
with increased requirements acc. to LAPP specification
colour: black, similar RAL 9005
Materials kg %
Plastic - Polyvinyl chloride (PVC) 0,02 30,99
Metal - Copper 0,05 69,01
Total 0,07 100,00
Packaging kg %
Packaging - Wood 0,01 100,00
Total incl. packaging 0,08 100,00
Technical data:
3 / 12
Electrical properties at 20 °C
Specific volume resistivity > 20 G ? x cm
Transfer impedance max. 250 m?/m (at 30 MHz)
Nominal voltage U0/ U: 300 / 500 V
Test voltage core / core: 4000 V AC
core / screen: 2000 V AC
Mechanical and thermal properties
Minimum bending radius occasional flexing: 20 x outer diameter
fixed installation: 6 x outer diameter
Temperature range occasional flexing: - 5°C up to +70°C max. conductor temp.
fixed installation: - 40°C up to +80°C max. conductor temp.
Torsional stress Torsion movement in wind turbine generators
TW-0 (5000 cycles at =+5 °C)
TW-1 (2000 cycles at =-20 °C)
±150 °/m at 1 revolution per minute
Flammability flame retardant acc. to IEC 60332-1-2 resp. EN 60332-1-2
UV resistance Acc. to EN 50525-1 cables with black sheath are suitable
for permanent outdoor use.
acc. to EN 50618
acc. to EN 50620
acc. to EN ISO 4892-2-2013, method A (change of colour allowed)
.
Tests acc. to IEC 60811 resp. EN 60811, EN 50395, EN 50396
General requirements These cables are conform to the EU-Directive 2014/35/EU
(Low Voltage Directive).
A part of these cables (see www.lappkabel.com/cpr) are classified
in accordance with the EU-Regulation no. 305/2011 (CPR).
Environmental information These cables meet the substance-specific requirements of the EU Directive 2011/65/EU (RoHS)
Market:
Norway
Reference service life, product
Expected lifetime 40 years, provided proper installation, load and ambient temperature.
Reference service life, building or construction works
40 years
LCA: Calculation rules
Declared unit:
1 m LAPP ÖLFLEX® CLASSIC 115 CY 4X0,5 BK Elnr 1025648
Cut-off criteria:
All major raw materials and all the essential energy is included. The production processes for raw materials and energy flows with very small
amounts (less than 1%) are not included. These cut-off criteria do not apply for hazardous materials and substances.
Allocation:
The allocation is made in accordance with the provisions of EN 15804. Incoming energy and water and waste production in-house is allocated
equally among all products through mass allocation. Effects of primary production of recycled materials is allocated to the main product in which
the material was used. The recycling process and transportation of the material is allocated to this analysis.
Data quality:
Specific data for the product composition are provided by the manufacturer. The data represent the production of the declared product and were
collected for EPD development in the year of study. Background data is based on EPDs according to EN 15804 and different LCA databases. The
data quality of the raw materials in A1 is presented in the table below.
Materials Source Data quality Year
Metal - Copper ecoinvent 3.6 Database 2019
Packaging - Wood ecoinvent 3.6 Database 2019
Plastic - Polyvinyl chloride (PVC) ecoinvent 3.6 Database 2019
4 / 12
System boundaries (X=included, MND=module not declared, MNR=module not relevant)
Construction Beyond the system
Product stage Use stage End of life stage
installation stage boundaries
A1 A2 A3 A4 A5 B1 B2 B3 B4 B5 B6 B7 C1 C2 C3 C4 D
X X X X X MND MND MND MND MND X MND X X X X X
System boundary:
1m LAPP ÖLFLEX® CLASSIC 115 CY 4X0,5 BK Elnr 1025648
The flowchart below illustrates the system boundaries of the analysis:
Additional technical information:
The article 1136514 ÖLFLEX® CLASSIC 115 CY 4X0,5 BK represents the product with the highest expenditure of raw materials and energy
consumption during manufacturing of all the following products from the same product family:
Elnr: Articelnr:
1025644 1136510
1025645 1136511
1025646 1136512
1025647 1136513
This EPD is only valid for the declared product.
waR slairetam tropsnarT gnirutcafunaM tropsnarT ylbmessA e​sU ecnanetniaM riapeR tnemecalpeR tnemhsibrufeR lanoitarepO ygrene esu lanoitarepO esu retaw -eD noitcurtsnoc noitilomed tropsnarT etsaW gnissecorp lasopsiD -yrevoceR-esueR laitnetop-gnilcyceR
5 / 12
LCA: Scenarios and additional technical information
The following information describe the scenarios in the different modules of the EPD.
Module A4 = In A4, a transport distance from the production site to LAPP Norways warehouse in Drammen was included. A distance of 300 km
was also added as additional transport to market.
Modules A5 = 5 % product losses during installation are estimated by the company. No energy use has been quantified since installation in
buildings is often done by manual labour. Use of portable electrical devices (e.g., drill) usually have low energy requirements falling under the cut​off
criterion of 1%. Cable drums are reused and also assumed under the cut-off criterion of 1%.
Module C1 = de-construction in buildings is often done by manual labour. Use of portable electrical devices (e.g., drill) usually have low energy
requirements falling under the cut-off criterion of 1%.
Module C2 = 85 km is added as an average distance to the waste facility
Modules C3 and C4 = Waste treatment of the product follows the default values provided in EN 50693, Product Category Rules for life cycle
assessments of electronic and electrical products and systems, table G.4. This table specified how different types of raw materials used in A1 will
likely be treated during the end-of-life of the product. Waste treatments in C3 include material recycling and incineration with and without energy
recovery and fly ash extraction. Disposal in C4 consist of landfilling of different waste fractions and of ashes.
Module D = The recyclability of metals and plastics allows the producers a credit for the net scrap that is produced at the end of a product’s life.
The benefits from recycling of net scrap are described in formula from EN 15804:2012+A2:2019. Substitution of heat and electricity generated by
the incineration with energy recovery of plastic insulation and other parts is also calculated in module D.
Capacity utilisation Value
Transport from production place to user (A4) Distance (km) Fuel/Energy Consumption Unit
(incl. return) % (Liter/tonne)
Truck, over 32 tonnes, EURO 6 (km) 53,3 % 1956 0,023 l/tkm 44,99
Truck, over 32 tonnes, EURO 6 (km) 53,3 % 300 0,023 l/tkm 6,90
Assembly (A5) Unit Value
Waste, packaging, pallet, EUR wooden pallet,
single use, to average treatment (kg) - A5, inkl. 85 kg 0,0050
km transp.
Product loss during installation (percentage of
Units/DU 0,050
cable)
Operational energy (B6) Unit Value
Electricity, Norway (kWh) kWh 9,57
Capacity utilisation Value
Transport to waste processing (C2) Distance (km) Fuel/Energy Consumption Unit
(incl. return) % (Liter/tonne)
Truck, 16-32 tonnes, EURO 6 (km) 36,7 % 85 0,043 l/tkm 3,66
Waste processing (C3) Unit Value
Copper to recycling (kg) kg 0,029
Waste treatment of polyvinylchloride (PVC),
incineration with energy recovery and fly ash kg 0,011
extraction (kg)
Disposal (C4) Unit Value
Landfilling of plastic mixture (kg) kg 0,021
Landfilling of copper (kg) kg 0,019
Landfilling of ashes from incineration of
Polyvinylchloride (PVC), process per kg ashes and kg 0,0017
residues (kg)
Benefits and loads beyond the system
Unit Value
boundaries (D)
Substitution of electricity, in Norway (MJ) MJ 0,014
Substitution of primary copper with net scrap (kg) kg 0,034
Substitution of thermal energy, district heating, in
MJ 0,22
Norway (MJ)
6 / 12
LCA: Results
The LCA results are presented below for the declared unit defined on page 2 of the EPD document.
Environmental impact
Indicator Unit A1 A2 A3 A4 A5
GWP-total kg CO2 -eq 2,78E-01 7,63E-03 2,51E-02 1,40E-02 2,77E-02
GWP-fossil kg CO2 -eq 2,81E-01 7,62E-03 2,35E-02 1,40E-02 2,01E-02
GWP-biogenic kg CO2 -eq -2,64E-03 3,15E-06 1,57E-03 5,98E-06 7,53E-03
GWP-luluc kg CO2 -eq 2,94E-04 2,71E-06 1,44E-05 4,25E-06 1,73E-05
ODP kg CFC11 -eq 4,47E-08 1,73E-09 7,58E-09 3,36E-09 4,22E-09
AP mol H+ -eq 1,14E-02 2,19E-05 8,09E-05 4,49E-05 5,77E-04
EP-FreshWater kg P -eq 9,29E-05 6,09E-08 5,80E-07 1,11E-07 4,66E-06
EP-Marine kg N -eq 7,94E-04 4,33E-06 1,77E-05 9,84E-06 4,27E-05
EP-Terrestial mol N -eq 1,16E-02 4,85E-05 1,68E-04 1,10E-04 6,03E-04
POCP kg NMVOC -eq 2,90E-03 1,86E-05 4,67E-05 4,31E-05 1,56E-04
ADP-minerals&metals1 kg Sb-eq 1,29E-04 2,11E-07 3,71E-07 2,49E-07 5,17E-06
ADP-fossil1 MJ 4,20E+00 1,15E-01 1,65E+00 2,27E-01 3,70E-01
WDP1 m3 1,73E+01 1,11E-01 2,50E+01 1,74E-01 2,20E+00
Indicator Unit B6 C1 C2 C3 C4 D
GWP-total kg CO2 -eq 9,32E-01 0 9,87E-04 2,20E-02 3,15E-03 -8,48E-02
GWP-fossil kg CO2 -eq 9,03E-01 0 9,86E-04 2,20E-02 3,15E-03 -8,43E-02
GWP-biogenic kg CO2 -eq 2,50E-02 0 4,08E-07 8,98E-06 4,20E-07 -3,88E-04
GWP-luluc kg CO2 -eq 3,72E-03 0 3,51E-07 1,72E-06 2,08E-07 -1,32E-04
ODP kg CFC11 -eq 6,19E-08 0 2,23E-10 7,24E-10 1,73E-10 -9,40E-05
AP mol H+ -eq 7,05E-03 0 2,83E-06 1,27E-05 5,00E-06 -1,39E-02
EP-FreshWater kg P -eq 6,49E-05 0 7,88E-09 6,49E-08 1,32E-08 -9,40E-05
EP-Marine kg N -eq 7,75E-04 0 5,61E-07 3,11E-06 4,26E-06 -5,76E-04
EP-Terrestial mol N -eq 1,01E-02 0 6,27E-06 3,34E-05 1,93E-05 -8,91E-03
POCP kg NMVOC -eq 2,71E-03 0 2,40E-06 9,44E-06 5,94E-06 -2,42E-03
ADP-minerals&metals1 kg Sb-eq 6,73E-05 0 2,72E-08 4,64E-08 5,07E-09 -7,81E-05
ADP-fossil1 MJ 1,23E+01 0 1,49E-02 2,90E-02 1,40E-02 -7,60E-01
WDP1 m3 2,15E+03 0 1,44E-02 5,92E-01 2,53E-01 4,31E+00
GWP-total = Global Warming Potential total; GWP-fossil = Global Warming Potential fossil fuels; GWP-biogenic = Global Warming Potential biogenic; GWP-luluc =
Global Warming Potential land use and land use change; ODP = Depletion potential of the stratospheric ozone layer; AP = Acidification potential, Accumulated
Exceedance; EP-freshwater = Eutrophication potential, fraction of nutrients reaching freshwater end compartment: EP-marine = Eutrophication potential, fraction of
nutrients reaching marine end compartment; EP-terrestrial = Eutrophication potential, Accumulated Exceedance; POCP = Formation potential of tropospheric ozone;
ADP-minerals&metals = Abiotic depletion potential for non-fossil resources; ADP-fossil = Abiotic depletion for fossil resources potential; WDP = Water (user)
deprivation potential, deprivation-weighted water consumption
"Reading example: 9,0 E-03 = 9,0*10-3 = 0,009"
*INA Indicator Not Assessed
1. The results of this environmental impact indicator shall be used with care as the uncertainties on these results are high or as there is limited experienced with the
indicator
Remarks to environmental impacts
7 / 12
Additional environmental impact indicators
Indicator Unit A1 A2 A3 A4 A5
PM Disease incidence 3,31E-08 4,67E-10 4,91E-10 1,28E-09 1,84E-09
IRP2 kgBq U235 -eq 1,64E-02 5,04E-04 1,63E-02 9,90E-04 1,80E-03
ETP-fw1 CTUe 1,38E+02 8,54E-02 5,94E-01 1,66E-01 7,40E+00
HTP-c1 CTUh 2,44E-09 0,00E+00 1,80E-11 0,00E+00 1,22E-10
HTP-nc1 CTUh 1,84E-07 9,30E-11 4,46E-10 1,60E-10 9,14E-09
SQP1 dimensionless 3,54E+00 8,06E-02 9,68E-02 2,60E-01 2,10E-01
Indicator Unit B6 C1 C2 C3 C4 D
PM Disease incidence 5,06E-08 0 6,00E-11 8,30E-11 8,10E-11 -2,85E-08
IRP2 kgBq U235 -eq 2,24E-01 0 6,51E-05 1,41E-04 8,10E-05 -1,04E-03
ETP-fw1 CTUe 5,62E+01 0 1,10E-02 1,39E+00 1,21E+01 -1,28E+02
HTP-c1 CTUh 2,68E-09 0 0,00E+00 3,00E-12 0,00E+00 -1,81E-09
HTP-nc1 CTUh 6,31E-08 0 1,20E-11 3,27E-10 2,80E-11 -1,55E-07
SQP1 dimensionless 6,21E+00 0 1,04E-02 1,06E-02 3,83E-02 -1,75E+00
PM = Particulate Matter emissions; IRP = Ionizing radiation – human health; ETP-fw = Eco toxicity – freshwater; HTP-c = Human toxicity – cancer effects; HTP-nc =
Human toxicity – non cancer effects; SQP = Potential Soil Quality Index (dimensionless)
"Reading example: 9,0 E-03 = 9,0*10-3 = 0,009"
*INA Indicator Not Assessed
1. The results of this environmental impact indicator shall be used with care as the uncertainties on these results are high or as there is limited experienced with the
indicator
2. This impact category deals mainly with the eventual impact of low dose ionizing radiation on human health of the nuclear fuel cycle. It does not consider effects due
to possible nuclear accidents, occupational exposure nor due to radioactive waste disposal in underground facilities. Potential ionizing radiation from the soil, from
radon and from some construction materials is also not measured by this indicator.
8 / 12
Resource use
Indicator Unit A1 A2 A3 A4 A5
PERE MJ 8,01E-01 1,65E-03 2,51E-01 2,85E-03 5,41E-02
PERM MJ 6,94E-02 0,00E+00 0,00E+00 0,00E+00 -6,59E-02
PERT MJ 8,70E-01 1,65E-03 2,51E-01 2,85E-03 -1,19E-02
PENRE MJ 3,73E+00 1,15E-01 1,65E+00 2,27E-01 3,23E-01
PENRM MJ 4,73E-01 0,00E+00 0,00E+00 0,00E+00 2,39E-02
PENRT MJ 4,20E+00 1,15E-01 1,65E+00 2,27E-01 3,47E-01
SM kg 8,29E-03 0,00E+00 0,00E+00 0,00E+00 4,28E-04
RSF MJ 1,99E-02 5,90E-05 1,81E-03 9,97E-05 1,13E-03
NRSF MJ 5,49E-04 2,11E-04 4,63E-03 3,34E-04 3,19E-04
FW m3 5,05E-03 1,23E-05 1,53E-03 2,58E-05 3,90E-04
Indicator Unit B6 C1 C2 C3 C4 D
PERE MJ 1,60E+02 0 2,13E-04 3,70E-03 1,37E-03 -4,11E-01
PERM MJ 0,00E+00 0 0,00E+00 0,00E+00 0,00E+00 0,00E+00
PERT MJ 1,60E+02 0 2,13E-04 3,70E-03 1,37E-03 -4,11E-01
PENRE MJ 1,23E+01 0 1,49E-02 2,90E-02 1,40E-02 -7,59E-01
PENRM MJ 0,00E+00 0 0,00E+00 -9,25E-01 0,00E+00 0,00E+00
PENRT MJ 1,23E+01 0 1,49E-02 -8,96E-01 1,40E-02 -7,59E-01
SM kg 0,00E+00 0 0,00E+00 0,00E+00 1,15E-06 2,43E-02
RSF MJ 1,25E-01 0 7,63E-06 6,69E-05 2,92E-05 2,29E-03
NRSF MJ 3,12E-01 0 2,73E-05 0,00E+00 4,52E-05 -1,77E-03
FW m3 1,19E+00 0 1,59E-06 6,94E-04 1,71E-05 -2,17E-03
PERE = Use of renewable primary energy excluding renewable primary energy resources used as raw materials; PERM = Use of renewable primary energy resources used
as raw materials; PERT = Total use of renewable primary energy resources; PENRE = Use of non renewable primary energy excluding non-renewable primary energy
resources used as raw materials; PENRM = Use of non renewable primary energy resources used as raw materials; PENRT = Total use of non renewable primary energy
resources; SM = Use of secondary materials; RSF = Use of renewable secondary fuels; NRSF = Use of non-renewable secondary fuels; FW = Net use of fresh water
"Reading example: 9,0 E-03 = 9,0*10-3 = 0,009"
*INA Indicator Not Assessed
9 / 12
End of life - Waste
Indicator Unit A1 A2 A3 A4 A5
HWD kg 2,90E-03 5,94E-06 3,33E-03 1,24E-05 3,73E-04
NHWD kg 1,05E-01 5,61E-03 1,60E-02 1,97E-02 1,47E-02
RWD kg 1,51E-05 7,85E-07 2,10E-05 1,55E-06 2,02E-06
Indicator Unit B6 C1 C2 C3 C4 D
HWD kg 7,91E-03 0 7,69E-07 0,00E+00 8,93E-04 -9,41E-04
NHWD kg 9,50E-01 0 7,25E-04 0,00E+00 4,30E-02 -4,04E-02
RWD kg 1,10E-04 0 1,02E-07 0,00E+00 8,39E-08 -9,30E-07
HWD = Hazardous waste disposed; NHWD = Non-hazardous waste disposed; RWD = Radioactive waste disposed
"Reading example: 9,0 E-03 = 9,0*10-3 = 0,009"
*INA Indicator Not Assessed
End of life - Output flow
Indicator Unit A1 A2 A3 A4 A5
CRU kg 0,00E+00 0,00E+00 0,00E+00 0,00E+00 0,00E+00
MFR kg 0,00E+00 0,00E+00 1,21E-02 0,00E+00 2,02E-03
MER kg 0,00E+00 0,00E+00 1,43E-02 0,00E+00 5,67E-03
EEE MJ 0,00E+00 0,00E+00 8,73E-03 0,00E+00 4,42E-03
EET MJ 0,00E+00 0,00E+00 1,32E-01 0,00E+00 6,69E-02
Indicator Unit B6 C1 C2 C3 C4 D
CRU kg 0,00E+00 0 0,00E+00 0,00E+00 0,00E+00 0,00E+00
MFR kg 0,00E+00 0 0,00E+00 2,94E-02 1,93E-06 -9,50E-04
MER kg 0,00E+00 0 0,00E+00 1,10E-02 4,72E-08 -1,25E-04
EEE MJ 0,00E+00 0 0,00E+00 1,13E-02 3,06E-06 -3,07E-04
EET MJ 0,00E+00 0 0,00E+00 1,70E-01 4,63E-05 -4,64E-03
CRU = Components for re-use; MFR = Materials for recycling; MER = Materials for energy recovery; EEE = Exported energy electrical; EET = Exported energy thermal
"Reading example: 9,0 E-03 = 9,0*10-3 = 0,009"
*INA Indicator Not Assessed
Biogenic Carbon Content
Indicator Unit At the factory gate
Biogenic carbon content in product kg C 0,00E+00
Biogenic carbon content in accompanying packaging kg C 2,07E-03
Note: 1 kg biogenic carbon is equivalent to 44/12 kg CO2
10 / 12
Additional requirements
Greenhouse gas emissions from the use of electricity in the manufacturing phase
National production mix from import, low voltage (production of transmission lines, in addition to direct emissions and losses in grid) of applied
electricity for the manufacturing process (A3).
Electricity mix Source Amount Unit
Electricity, Norway (kWh) ecoinvent 3.6 24,33 g CO2-eq/kWh
Electricity, France (kWh) ecoinvent 3.6 94,37 g CO2-eq/kWh
Dangerous substances
The product contains no substances given by the REACH Candidate list.
Indoor environment
No effect on indoor environment.
Additional Environmental Information
Additional environmental impact indicators required in NPCR Part A for construction products
Indicator Unit A1 A2 A3 A4 A5
GWPIOBC kg CO2 -eq 2,86E-01 7,63E-03 2,48E-02 1,40E-02 2,04E-02
Indicator Unit B6 C1 C2 C3 C4 D
GWPIOBC kg CO2 -eq 9,30E-01 0 9,86E-04 2,21E-02 2,03E-03 -4,07E-02
GWP-IOBC: Global warming potential calculated according to the principle of instantaneous oxidation. In order to increase the transparency of biogenic carbon​
contribution to climate impact, the indicator GWP-IOBC is required as it declares climate impacts calculated according to the principle of instantaneous oxidation.​
GWP-IOBC is also referred to as GWP-GHG in context to Swedish public procurement legislation.
11 / 12
Bibliography
ISO 14025:2010. Environmental labels and declarations - Type III environmental declarations - Principles and procedures. International
Organization for Standardization.
ISO 14044:2006. Environmental management - Life cycle assessment - Requirements and guidelines. International Organization for
Standardization.
EN 15804:2012+A2:2019. Environmental product declaration - Core rules for the product category of construction products. European
Committee for Standardization.
ISO 21930:2017. Sustainability in buildings and civil engineering works - Core rules for environmental product declarations of construction
products. International Organization for Standardization.
EN 50693:2019. Product category rules for life cycle assessments of electronic and electrical products and systems. European Committee for
Standardization.
Ecoinvent v3, 2019. Allocation, cut-off by classification. Swiss Centre of Life Cycle Inventories.
Iversen et al., (2021). eEPD v2021.09, background information for EPD generator tool system verification, LCA.no. Report number: 07.21. System
verification report.
Philis et al., (2022). EPD generator for NPCR 027 part B for electrical wires and cables, background information for EPD generator application and
LCA data, LCA.no Report number: 03.22. PCR verification report.
EPD Norway (2022). NPCR Part A: Construction products and services. The Norwegian EPD foundation. Version 2.0 published 24.03.2021.
EPD Norway (2022). NPCR 027 Part B for electrical cables and wires. The Norwegian EPD foundation. Version 2.0 published 01.03.2022.
Program operator and publisher Phone: +47 977 22 020
The Norwegian EPD Foundation e-mail: post@epd-norge.no
Post Box 5250 Majorstuen, 0303 Oslo, Norway web: www.epd-norge.no
Owner of the declaration: Phone: 91597046
Lapp Norway AS e-mail: petter.dahl@lapp.com
Eikringen 11, 3036 Drammen, Norway web: no.lappgroup.com
Author of the Life Cycle Assessment Phone: +47 916 50 916
LCA.no AS e-mail: post@lca.no
Dokka 6A, 1671 Kråkerøy, Norway web: www.lca.no
Developer of EPD generator Phone: +47 916 50 916
LCA.no AS e-mail: post@lca.no
Dokka 6A, 1671 Kråkerøy, Norway web: www.lca.no
ECO Platform web: www.eco-platform.org
ECO Portal web: ECO Portal
12 / 12
