Environmental product declaration
in accordance with ISO 14025 and EN 15804+A2
amina S – AST100/20
Owner of the declaration: Program operator:
Amina Distribution AS The Norwegian EPD Foundation
Product: Declaration number:
amina S – AST100/20
NEPD-5975-5242-EN
Declared unit:
1 pcs Registration number:
This declaration is based on Product Category Rules: NEPD-5975-5242-EN
CEN Standard EN 15804:2012+A2:2019, EN 50693:2019
Issue date: 01.02.2024
and PCR EPD Italy 007 serves as core PCR
The Norwegian EPD Foundation
PCR EPD Italy 017 - Electronic and electrical products and Valid to: 01.02.2029
systems - Charging stations
EPD software:
LCAno EPD generator ID: 151816
1 / 14
General information
Product Owner of the declaration:
amina S – AST100/20 Amina Distribution AS
Contact person: Fredrik Lima
Phone: +47 45441014
e-mail: fredrik@aminacharging.com
Program operator: Manufacturer:
Post Box 5250 Majorstuen, 0303 Oslo, Norway Amina Distribution AS
The Norwegian EPD Foundation Grenseveien 21
Phone: +47 23 08 80 00 4313 Sandnes, Norway
web: post@epd-norge.no
Declaration number: Place of production:
NEPD-5975-5242-EN Production site Topro Elektronikk (Norway
Rambekkvegen 7
2816 Gjøvik, Norway
This declaration is based on Product Category Rules: Management system:
CEN Standard EN 15804:2012+A2:2019, EN 50693:2019 and PCR
EPD Italy 007 serves as core PCR
PCR EPD Italy 017 - Electronic and electrical products and systems -
Charging stations
Statement of liability: Organisation no:
The owner of the declaration shall be liable for the underlying 928228096
information and evidence. EPD Norway shall not be liable with respect
to manufacturer information, life cycle assessment data and
evidences.​
Declared unit: Issue date: 01.02.2024
1 pcs amina S – AST100/20
Declared unit with option: Valid to: 01.02.2029
A1,A2,A3,A4,A5,B6,C1,C2,C3,C4,D
Year of study:
2023
Functional unit: Comparability:
1 pcs of EVSE, installed and used during a service life of 20 years, EPD of construction products may not be comparable if they not
including waste treatment at end of life. comply with EN 15804 and seen in a building context.
General information on verification of EPD from EPD tools: Development and verification of EPD:
Independent verification of data, other environmental information The declaration is created using EPD tool lca.tools ver EPD2022.03,
and the declaration according to ISO 14025:2010, § 8.1.3 and § 8.1.4. developed by LCA.no. The EPD tool is integrated in the company's
Verification of each EPD is made according to EPD-Norway’s management system, and has been approved by EPD Norway.
guidelines for verification and approval requiring that tools are i)
integrated into the company's environmental management system, ii) Developer of EPD: Fredrik Lima
the procedures for use of the EPD tool are approved by EPD-Norway,
Reviewer of company-specific input data and EPD:​ Limin Yang
and iii) the process is reviewed annually by an independent third
party verifier. See Appendix G of EPD-Norway's General Programme
Instructions for further information on EPD tools
Verification of EPD tool: Approved:
Independent third party verification of the EPD tool, background data
and test-EPD in accordance with EPDNorway's procedures and
guidelines for verification and approval of EPD tools.
Third party verifier:
Elisabet Amat, GREENIZE projects
(no signature required)
2 / 14
Product
Product description:
amina S is intended for charging electrically powered vehicles. It is classified as a mode-3 EVSE that can be used by ordinary persons. The product
must be securely mounted on a sturdy surface. It may only be operated within the approved operating parameters and under specified
environmental conditions.
Product specification
amina S is the small, fast, and smart charger that gives you complete control over charging speed and energy consumption. With its lightweight
and flexible fixed cable, you can charge up to 22kW.
Materials kg %
Electronic - Capacitor 0,00 0,09
Electronic - Charging Cable 1,48 56,67
Electronic - Connector 0,23 8,75
Electronic - Diode 0,00 0,02
Electronic - Inductor 0,01 0,26
Electronic - Integrated circuit 0,00 0,05
Electronic - LED chip 0,00 0,00
Electronic - Printed wiring board 0,08 3,15
Electronic - Resistor 0,00 0,10
Electronic - Solder material 0,00 0,12
Electronic - Transistor 0,00 0,03
Electronic - Unspecified 0,00 0,04
Electronic component 0,08 2,88
Ethylene propylene diene monomer (EPDM) 0,00 0,08
Metal - Steel 0,02 0,94
Metal/plastic - Stainless steel and EVA 0,00 0,09
Plastic - Plexiglass (PMMA) 0,00 0,15
Plastic - Polycarbonate (PC) 0,00 0,08
Plastic compound - PC and ABS 0,69 26,44
Product label - supercalendered 0,00 0,01
Tape - Polyester 0,00 0,05
Total 2,61
Packaging kg %
Packaging - Cardboard 0,45 87,74
Packaging - Paper 0,06 12,26
Total incl. packaging 3,12
Technical data:
Dimensions
264mm x 112mm x 89mm
Weight
1,0 kg w/o cable
2,4 kg w/ 6m 3-phase 20A cable
3,4 kg w/ 6m 3-phase 32A cable
Operating temperature
-30°C to +40°C
Electrical rating
Class I equipment
Overvoltage category III (4 kV)
Idc = 6 mA, Im = 500 A, Inc = 3kA
3x 230/400V 50Hz AC
20A (AST 1xx/20)
32A (AST 1xx/32)
Number of poles = 4
Charging cable
Fixed cable included (replaceable)
Type 2 plug (EN 62196)
AST 100/20: 6m 3-phase 20A
AST 100/32: 6m 3-phase 32A
Charging power 20A variant
3-phase output: 3,7 – 13,8 kW
3 / 14
1-phase output: 1,4 – 4,6 kW
Charging power 32A variant
3-phase output: 3,7 – 22,0 kW
1-phase output: 1,4 – 7,4 kW
Integrated energy-meter
1 or 3-phase
±3 % accuracy
Communications interface
Bluetooth LE and Zigbee
Frequency band: 2400 – 2483,5 MHz
Maximum output power: 10mW
Installation environment
Indoor and outdoor use (IP54)
Private and public locations (IK08)
Wall or pole mounted
Min 90cm installation height
Installation
Permanently connected
Three-phase w/ neutral (TN/TT)
Single-phase (TN/TT/IT)
4 – 16mm cable diameter
Power supply terminals
Single core or stranded wires
1,5 – 6mm2 w/ ferrules
1,5 – 10mm2 w/o ferrules
Strip wires 12 – 14mm
Integrated RCD
RDC-DD (6mA DC)
Regulations and standards
RED 2014/53/EU
EN IEC 62311:2020
EN IEC 61851-1:2019
EN 62196-1:2014
EN 62196-2:2012+A11:2013+A12:2014
IEC 62955:2018*
EN IEC 61851-21-2:2021
EN 301 489-1 v2.2.3
EN 301 489-17 v3.2.4
EN 300 328 v2.2.2
RoHS 2011/65/EU
EN IEC 63000:2018
*Clause 8.1.2: mechanically coupled switches in single phase installations, electronically coupled in three phase installations. See
aminacharging.com/compliance for more information.
Market:
Nordics
Reference service life, product
20 years.
Reference service life, building or construction works
Not applicable.
LCA: Calculation rules
Declared unit:
1 pcs amina S – AST100/20
4 / 14
Cut-off criteria:
All major raw materials and all the essential energy is included. The production processes for raw materials and energy flows with very small
amounts (less than 1%) are not included. These cut-off criteria do not​ apply for hazardous materials and substances.
Allocation:
The allocation is made in accordance with the provisions of EN 15804. Incoming energy and water and waste production in-house is allocated
equally among all products through mass allocation. Effects of primary production of recycled materials is allocated to the main product in which
the material was used. The recycling process and transportation of the material is allocated to this analysis.
Data quality:
Specific data for the product composition are provided by the manufacturer. The data represent the production of the declared product and were
collected for EPD development in the year of study. Background data is based on EPDs according to EN 15804 and different LCA databases. The
data quality of the raw materials in A1 is presented in the table below.
Materials Source Data quality Year
Electronic - Capacitor ecoinvent 3.6 Database 2019
Database +
Electronic - Charging Cable Ecoinvent 3.6 + Supplier Information Supplier 2019
Information
Electronic - Connector Ecoinvent 3.6 Database 2019
Electronic - Diode ecoinvent 3.6 Database 2019
Electronic - Inductor ecoinvent 3.6 Database 2019
Electronic - Integrated circuit ecoinvent 3.6 Database 2019
Scientific
Electronic - LED chip Scholand et al. (2012) + Ecoinvent 3.6 literature + 2017
database
Electronic - Printed wiring board Modified ecoinvent 3.6 Database 2019
Electronic - Resistor ecoinvent 3.6 Database 2019
Electronic - Solder material ecoinvent 3.6 Database 2019
Electronic - Transistor ecoinvent 3.6 Database 2019
Electronic - Unspecified ecoinvent 3.6 Database 2019
Database +
Electronic component Ecoinvent 3.6 + Supplier Information Supplier 2019
Information
Ethylene propylene diene monomer (EPDM) ecoinvent 3.6 Database 2019
Metal - Steel Ecoinvent 3.6 Database 2019
Supplier data +
Metal/plastic - Stainless steel and EVA Product composition + Ecoinvent 3.6 2019
database
Packaging - Cardboard Modified ecoinvent 3.6 Database 2019
Packaging - Paper ecoinvent 3.6 Database 2019
Supplier data +
Plastic - Plexiglass (PMMA) Product composition + ecoinvent 3.6 2019
database
Plastic - Polycarbonate (PC) ecoinvent 3.6 Database 2019
Plastic compound - PC and ABS Ecoinvent 3.6 Database 2019
Product label - supercalendered Ecoinvent 3.6 Database 2019
Tape - Polyester ecoinvent 3.6 Database 2019
5 / 14
System boundaries (X=included, MND=module not declared, MNR=module not relevant)
Construction Beyond the system
Product stage Use stage End of life stage
installation stage boundaries
A1 A2 A3 A4 A5 B1 B2 B3 B4 B5 B6 B7 C1 C2 C3 C4 D
X X X X X MND MND MND MND MND X MND X X X X X
System boundary:
Additional technical information:
waR slairetam tropsnarT gnirutcafunaM tropsnarT ylbmessA e​sU ecnanetniaM riapeR tnemecalpeR tnemhsibrufeR lanoitarepO ygrene esu lanoitarepO esu retaw -eD noitcurtsnoc noitilomed tropsnarT etsaW gnissecorp lasopsiD -yrevoceR-esueR laitnetop-gnilcyceR
6 / 14
LCA: Scenarios and additional technical information
The following information describe the scenarios in the different modules of the EPD.
Module A4 = An average distance between the factory and the market is considered.
Modules A5 = installation is done by manual labor. The use of portable electrical devices such as drills usually have low energy requirements falling
under the cut-off criterion of 1% and are therefore neglected. No product scraps are generated during installation, but the end-of-life treatment of
packaging is accounted for in this module.
Module B6 = The operational energy use of the charging station is calculated based on the methodology provided in EPD Italy PCR 017 for
charging stations (details are provided in section 4.2.3.5). Calculations focus on the energy consumed by the charging station during its entire
service life. It is important to note that impacts related to electricity delivered to the charging vehicle are outside of the system boundaries of this
EPD. Use phase considers only the energy absorbed by the charging station to keep operating and ready (e.g., display, LEDs) to transfer electric
power to the connected vehicle. The energy absorbed is calculated as follows:
- Power consumed by the charging station (Puse) = 0.78 watt
- Reference service life of the charging station (RSL) = 20 years (standard value)
- Hours per year = 8760 hours (standard value)
- Conversion factor from watt to kilowatt = 1000 (standard value)
Module C1 = De-installation is done by manual labor. The use of portable electrical devices such as drills usually have low energy requirements
falling under the cut-off criterion of 1% and are therefore neglected.
Module C2 = An average distance between the market and the waste treatment facility is considered. It is assumed that transport of charging
stations after the use phase is done by the end user with an average petrol car.
Modules C3 and C4 = Waste treatment of the product follows the default values provided in EN 50693, Product Category Rules for life cycle
assessments of electronic and electrical products and systems, table G.4. This table specified how different types of raw materials used in A1 will
likely be treated during the end-of-life of the product. Waste treatments in C3 include material recycling and incineration with energy recovery and
fly ash extraction. Disposal in C4 consist of landfilling of different waste fractions and of ashes.
Module D = The recyclability of metals, plastics, and electronic components allows the producers a credit for the net scrap that is produced at the
end of a product’s life. The benefits from recycling of net scrap are described in formula from EN 15804:2012+A2:2019. Substitution of heat and
electricity generated by the incineration with energy recovery of plastic insulation and other parts is also calculated in module D.
Capacity utilisation Value
Transport from production place to user (A4) Distance (km) Fuel/Energy Consumption Unit
(incl. return) % (Liter/tonne)
Truck, 16-32 tonnes, EURO 6 (km) - Europe 36,7 % 350 0,043 l/tkm 15,05
Assembly (A5) Unit Value
Waste, packaging, corrugated board box, to
kg 0,45
average treatment - A5 including transport (kg)
Waste, packaging, paper printed, to average
kg 0,06
treatment - A5 including transport (kg)
Operational energy (B6) Unit Value
Electricity, Nordic (kWh) kWh/DU 136,66
Capacity utilisation Value
Transport to waste processing (C2) Distance (km) Fuel/Energy Consumption Unit
(incl. return) % (Liter/tonne)
Passenger car, large size, petrol, EURO 5 (km) -
% 15 0,625 l/tkm 9,38
Europe
Waste processing (C3) Unit Value
Copper to recycling (kg) kg 0,39
Non-ferrous metal to recycling (kg) kg 0,03
Steel to recycling (kg) kg 0,03
Waste treatment of plastic mixture, incineration
kg 0,76
with energy recovery and fly ash extraction (kg)
Waste treatment per kg electronics scrap from
PWB, with components, recycling of metals C3 kg 0,17
(kg)
Waste treatment per kg used electronic cable,
kg 1,54
manual seperation (kg)
Waste treatment per kg used PWB, shredding and
kg 0,35
separation - C3 (kg)
7 / 14
Disposal (C4) Unit Value
Landfilling of ashes from incineration of Plastic
kg 0,03
mixture, process per kg ashes and residues (kg)
Landfilling of copper (kg) kg 0,26
Landfilling of hazardous waste (kg) kg 0,17
Landfilling of municipal solid waste (kg) kg 0,00
Landfilling of non-ferrous metal (kg) kg 0,02
Landfilling of plastic mixture (kg) kg 0,76
Landfilling of steel (kg) kg 0,01
Benefits and loads beyond the system
Unit Value
boundaries (D)
Substitution of electricity, in Norway (MJ) MJ 1,17
Substitution of primary copper with net scrap (kg) kg 0,38
Substitution of primary metals with net scrap
kg 0,05
from PWB, with components (kg)
Substitution of primary other non-ferrous metals
kg 0,03
with net scrap (kg)
Substitution of primary steel with net scrap (kg) kg 0,02
Substitution of thermal energy, district heating, in
MJ 17,73
Norway (MJ)
8 / 14
LCA: Results
The LCA results are presented below for the declared unit defined on page 2 of the EPD document.
Environmental impact
Indicator Unit A1 A2 A3 A4 A5
GWP-total kg CO2 -eq 5,74E+01 8,12E-01 5,80E-02 1,79E-01 8,83E-01
GWP-fossil kg CO2 -eq 5,79E+01 8,11E-01 5,42E-02 1,78E-01 8,31E-03
GWP-biogenic kg CO2 -eq -5,74E-01 3,17E-04 3,66E-03 7,38E-05 8,75E-01
GWP-luluc kg CO2 -eq 7,50E-02 3,17E-04 1,38E-04 6,35E-05 2,75E-06
ODP kg CFC11 -eq 4,17E-06 1,83E-07 3,83E-09 4,04E-08 1,76E-09
AP mol H+ -eq 1,11E+00 6,22E-03 2,94E-04 5,13E-04 3,94E-05
EP-FreshWater kg P -eq 1,76E-02 5,99E-06 2,44E-06 1,43E-06 6,83E-08
EP-Marine kg N -eq 1,45E-01 1,67E-03 5,03E-05 1,01E-04 1,30E-05
EP-Terrestial mol N -eq 1,83E+00 1,85E-02 5,58E-04 1,13E-03 1,41E-04
POCP kg NMVOC -eq 4,59E-01 5,25E-03 1,52E-04 4,35E-04 4,05E-05
ADP-minerals&metals1 kg Sb-eq 5,89E-02 1,99E-05 2,40E-06 4,93E-06 2,02E-07
ADP-fossil1 MJ 7,68E+02 1,20E+01 5,27E-01 2,70E+00 1,16E-01
WDP1 m3 1,61E+03 1,04E+01 7,24E+01 2,61E+00 1,47E-01
Indicator Unit B6 C1 C2 C3 C4 D
GWP-total kg CO2 -eq 1,99E+01 0,00E+00 1,21E-01 2,11E+00 1,30E-01 -3,95E+00
GWP-fossil kg CO2 -eq 1,86E+01 0,00E+00 1,21E-01 2,11E+00 1,28E-01 -3,93E+00
GWP-biogenic kg CO2 -eq 3,39E-01 0,00E+00 9,59E-05 7,02E-04 1,31E-03 -1,25E-02
GWP-luluc kg CO2 -eq 1,02E+00 0,00E+00 5,11E-05 5,89E-04 3,29E-04 -8,70E-03
ODP kg CFC11 -eq 2,01E-06 0,00E+00 2,17E-08 1,99E-08 5,41E-09 -7,49E-03
AP mol H+ -eq 8,56E-02 0,00E+00 4,17E-04 1,68E-03 2,64E-04 -3,36E-01
EP-FreshWater kg P -eq 1,23E-03 0,00E+00 2,08E-06 1,23E-05 1,81E-06 -2,04E-03
EP-Marine kg N -eq 1,35E-02 0,00E+00 6,24E-05 4,15E-04 1,60E-04 -1,59E-02
EP-Terrestial mol N -eq 1,82E-01 0,00E+00 7,18E-04 4,49E-03 7,37E-04 -2,28E-01
POCP kg NMVOC -eq 4,25E-02 0,00E+00 3,16E-04 1,17E-03 3,05E-04 -6,38E-02
ADP-minerals&metals1 kg Sb-eq 2,89E-04 0,00E+00 9,19E-06 1,92E-06 3,02E-07 -5,20E-03
ADP-fossil1 MJ 5,01E+02 0,00E+00 1,63E+00 3,51E+00 6,76E-01 -4,77E+01
WDP1 m3 3,88E+04 0,00E+00 1,90E+00 2,43E+01 4,24E+00 -5,28E+01
GWP-total = Global Warming Potential total; GWP-fossil = Global Warming Potential fossil fuels; GWP-biogenic = Global Warming Potential biogenic; GWP-luluc =
Global Warming Potential land use and land use change; ODP = Depletion potential of the stratospheric ozone layer; AP = Acidification potential, Accumulated
Exceedance; EP-freshwater = Eutrophication potential, fraction of nutrients reaching freshwater end compartment: EP-marine = Eutrophication potential, fraction of
nutrients reaching marine end compartment; EP-terrestrial = Eutrophication potential, Accumulated Exceedance; POCP = Formation potential of tropospheric ozone;
ADP-minerals&metals = Abiotic depletion potential for non-fossil resources; ADP-fossil = Abiotic depletion for fossil resources potential; WDP = Water (user)
deprivation potential, deprivation-weighted water consumption
"Reading example: 9,0 E-03 = 9,0*10-3 = 0,009"
*INA Indicator Not Assessed
1. The results of this environmental impact indicator shall be used with care as the uncertainties on these results are high or as there is limited experienced with the
indicator
Remarks to environmental impacts
9 / 14
Additional environmental impact indicators
Indicator Unit A1 A2 A3 A4 A5
PM Disease incidence 4,47E-06 5,13E-08 2,46E-09 1,09E-08 5,81E-10
IRP2 kgBq U235 -eq 2,43E+00 5,23E-02 7,93E-03 1,18E-02 4,98E-04
ETP-fw1 CTUe 1,63E+04 8,63E+00 2,15E+00 2,00E+00 1,55E-01
HTP-c1 CTUh 1,40E-07 0,00E+00 1,09E-10 0,00E+00 5,00E-12
HTP-nc1 CTUh 1,07E-05 8,73E-09 2,58E-09 2,18E-09 1,95E-10
SQP1 dimensionless 4,07E+02 7,54E+00 3,03E-01 1,89E+00 7,80E-02
Indicator Unit B6 C1 C2 C3 C4 D
PM Disease incidence 4,54E-07 0,00E+00 4,68E-09 1,08E-08 4,89E-09 -7,21E-07
IRP2 kgBq U235 -eq 1,14E+01 0,00E+00 6,62E-03 1,63E-02 2,08E-03 -1,59E-01
ETP-fw1 CTUe 6,28E+02 0,00E+00 2,20E+00 9,08E+00 1,78E+02 -2,71E+03
HTP-c1 CTUh 1,46E-08 0,00E+00 9,40E-11 3,06E-09 1,75E-10 -2,62E-08
HTP-nc1 CTUh 3,85E-07 0,00E+00 1,78E-09 1,78E-07 1,43E-09 -2,12E-06
SQP1 dimensionless 3,78E+02 0,00E+00 7,09E-01 7,14E-01 1,86E+00 -5,51E+01
PM = Particulate Matter emissions; IRP = Ionizing radiation – human health; ETP-fw = Eco toxicity – freshwater; HTP-c = Human toxicity – cancer effects; HTP-nc =
Human toxicity – non cancer effects; SQP = Potential Soil Quality Index (dimensionless)
"Reading example: 9,0 E-03 = 9,0*10-3 = 0,009"
*INA Indicator Not Assessed
1. The results of this environmental impact indicator shall be used with care as the uncertainties on these results are high or as there is limited experienced with the
indicator
2. This impact category deals mainly with the eventual impact of low dose ionizing radiation on human health of the nuclear fuel cycle. It does not consider effects due
to possible nuclear accidents, occupational exposure nor due to radioactive waste disposal in underground facilities. Potential ionizing radiation from the soil, from
radon and from some construction materials is also not measured by this indicator.
10 / 14
Resource use
Indicator Unit A1 A2 A3 A4 A5
PERE MJ 7,12E+01 1,59E-01 5,37E+00 3,86E-02 1,91E-03
PERM MJ 8,07E+00 0,00E+00 0,00E+00 0,00E+00 -4,59E+00
PERT MJ 7,93E+01 1,59E-01 5,37E+00 3,86E-02 -4,59E+00
PENRE MJ 7,10E+02 1,20E+01 5,27E-01 2,70E+00 1,16E-01
PENRM MJ 5,89E+01 0,00E+00 0,00E+00 0,00E+00 0,00E+00
PENRT MJ 7,69E+02 1,20E+01 5,27E-01 2,70E+00 1,16E-01
SM kg 1,11E-01 0,00E+00 0,00E+00 0,00E+00 0,00E+00
RSF MJ 1,15E+00 5,60E-03 4,35E-03 1,38E-03 6,35E-05
NRSF MJ 2,01E-01 2,15E-02 1,19E-02 4,94E-03 2,62E-04
FW m3 5,52E-01 1,19E-03 4,01E-02 2,88E-04 5,49E-05
Indicator Unit B6 C1 C2 C3 C4 D
PERE MJ 4,93E+02 0,00E+00 4,44E-02 4,19E-01 1,64E-01 -1,58E+01
PERM MJ 0,00E+00 0,00E+00 0,00E+00 0,00E+00 0,00E+00 0,00E+00
PERT MJ 4,93E+02 0,00E+00 4,44E-02 4,19E-01 1,64E-01 -1,58E+01
PENRE MJ 5,09E+02 0,00E+00 1,63E+00 3,51E+00 6,76E-01 -4,77E+01
PENRM MJ 0,00E+00 0,00E+00 0,00E+00 -5,96E+01 0,00E+00 0,00E+00
PENRT MJ 5,09E+02 0,00E+00 1,63E+00 -5,61E+01 6,76E-01 -4,77E+01
SM kg 0,00E+00 0,00E+00 0,00E+00 0,00E+00 5,24E-03 2,67E-01
RSF MJ 4,98E+00 0,00E+00 1,12E-03 8,60E-03 7,46E-04 2,57E-02
NRSF MJ 0,00E+00 0,00E+00 6,47E-03 -1,75E-04 3,27E-02 -4,28E-01
FW m3 2,24E+00 0,00E+00 3,54E-04 4,11E-03 5,61E-04 -6,02E-02
PERE = Use of renewable primary energy excluding renewable primary energy resources used as raw materials; PERM = Use of renewable primary energy resources used
as raw materials; PERT = Total use of renewable primary energy resources; PENRE = Use of non renewable primary energy excluding non-renewable primary energy
resources used as raw materials; PENRM = Use of non renewable primary energy resources used as raw materials; PENRT = Total use of non renewable primary energy
resources; SM = Use of secondary materials; RSF = Use of renewable secondary fuels; NRSF = Use of non-renewable secondary fuels; FW = Net use of fresh water
"Reading example: 9,0 E-03 = 9,0*10-3 = 0,009"
*INA Indicator Not Assessed
11 / 14
End of life - Waste
Indicator Unit A1 A2 A3 A4 A5
HWD kg 2,27E-01 6,02E-04 1,14E-02 1,39E-04 0,00E+00
NHWD kg 5,60E+00 5,14E-01 4,39E-02 1,31E-01 5,14E-01
RWD kg 2,22E-03 8,20E-05 4,30E-06 1,84E-05 0,00E+00
Indicator Unit B6 C1 C2 C3 C4 D
HWD kg 4,70E-02 0,00E+00 3,98E-04 8,63E-05 1,84E-01 -2,09E-02
NHWD kg 3,11E+00 0,00E+00 4,36E-02 1,16E-01 1,06E+00 -9,72E-01
RWD kg 5,25E-03 0,00E+00 9,82E-06 4,28E-06 1,82E-06 -1,37E-04
HWD = Hazardous waste disposed; NHWD = Non-hazardous waste disposed; RWD = Radioactive waste disposed
"Reading example: 9,0 E-03 = 9,0*10-3 = 0,009"
*INA Indicator Not Assessed
End of life - Output flow
Indicator Unit A1 A2 A3 A4 A5
CRU kg 0,00E+00 0,00E+00 0,00E+00 0,00E+00 0,00E+00
MFR kg 0,00E+00 0,00E+00 9,39E-02 0,00E+00 4,78E-01
MER kg 0,00E+00 0,00E+00 1,56E-01 0,00E+00 3,59E-02
EEE MJ 0,00E+00 0,00E+00 1,06E-01 0,00E+00 2,94E-02
EET MJ 0,00E+00 0,00E+00 1,60E+00 0,00E+00 4,45E-01
Indicator Unit B6 C1 C2 C3 C4 D
CRU kg 0,00E+00 0,00E+00 0,00E+00 0,00E+00 0,00E+00 0,00E+00
MFR kg 0,00E+00 0,00E+00 0,00E+00 4,47E-01 7,11E-05 -1,05E-02
MER kg 0,00E+00 0,00E+00 0,00E+00 7,63E-01 3,78E-05 -1,38E-03
EEE MJ 0,00E+00 0,00E+00 0,00E+00 1,17E+00 4,29E-04 -3,37E-03
EET MJ 0,00E+00 0,00E+00 0,00E+00 1,77E+01 6,49E-03 -5,10E-02
CRU = Components for re-use; MFR = Materials for recycling; MER = Materials for energy recovery; EEE = Exported energy electrical; EET = Exported energy thermal
"Reading example: 9,0 E-03 = 9,0*10-3 = 0,009"
*INA Indicator Not Assessed
Biogenic Carbon Content
Indicator Unit At the factory gate
Biogenic carbon content in product kg C 1,07E-04
Biogenic carbon content in accompanying packaging kg C 2,39E-01
Note: 1 kg biogenic carbon is equivalent to 44/12 kg CO2
12 / 14
Additional requirements
Greenhouse gas emissions from the use of electricity in the manufacturing phase
National production mix from import, low voltage (production of transmission lines, in addition to direct emissions and losses in grid) of applied
electricity for the manufacturing process (A3).
Electricity mix Data source Amount Unit
Electricity, Norway (kWh) ecoinvent 3.6 24,33 g CO2-eq/kWh
Dangerous substances
The product contains no substances given by the REACH Candidate list.
Indoor environment
Additional Environmental Information
Additional environmental impact indicators required in NPCR Part A for construction products
Indicator Unit A1 A2 A3 A4 A5
GWPIOBC kg CO2 -eq 5,82E+01 8,12E-01 5,64E-02 1,79E-01 8,32E-03
Indicator Unit B6 C1 C2 C3 C4 D
GWPIOBC kg CO2 -eq 2,70E+01 0,00E+00 1,21E-01 2,11E+00 1,33E-01 -3,49E+00
GWP-IOBC: Global warming potential calculated according to the principle of instantaneous oxidation. In order to increase the transparency of biogenic carbon​
contribution to climate impact, the indicator GWP-IOBC is required as it declares climate impacts calculated according to the principle of instantaneous oxidation.​
GWP-IOBC is also referred to as GWP-GHG in context to Swedish public procurement legislation.
13 / 14
Bibliography
ISO 14025:2010. Environmental labels and declarations - Type III environmental declarations - Principles and procedures. International
Organization for Standardization.
ISO 14044:2006. Environmental management - Life cycle assessment - Requirements and guidelines. International Organization for
Standardization.
EN 15804:2012+A2:2019. Environmental product declaration - Core rules for the product category of construction products. European
Committee for Standardization.
ISO 21930:2017. Sustainability in buildings and civil engineering works - Core rules for environmental product declarations of construction
products. International Organization for Standardization.
EN 50693:2019. Product category rules for life cycle assessments of electronic and electrical products and systems. European Committee for
Standardization.
Ecoinvent v3, 2019. Allocation, cut-off by classification. Swiss Centre of Life Cycle Inventories.
Iversen et al., (2021). eEPD v2021.09, background information for EPD generator tool system verification, LCA.no. Report number: 07.21. System
verification report.
Babwah & Philis (2023). EPD generator for EPD Italy PCR 017 part B for charging stations, background information for EPD generator application
and LCA data, LCA.no. Report number: 11.23. PCR verification report.
EPD Italy (2020). PCR EPD Italy 007 Part A for electronic and electrical products and systems. EPD Italy. Version 3, issue 13-01-2023 and valid
until 19-01-2025.
EPD Italy (2020). PCR EPD Italy 017 Part B for charging stations. EPD Italy. Version 1, issue 19-10-2020 and valid until 19-10-2025.
Program operator and publisher Phone: +47 23 08 80 00
The Norwegian EPD Foundation e-mail: post@epd-norge.no
Post Box 5250 Majorstuen, 0303 Oslo, Norway web: www.epd-norge.no
Owner of the declaration: Phone: +47 45441014
Amina Distribution AS e-mail: fredrik@aminacharging.com
Grenseveien 21, 4313 Sandnes web: https://aminacharging.com/
Author of the Life Cycle Assessment Phone: +47 916 50 916
LCA.no AS e-mail: post@lca.no
Dokka 6B, 1671 web: www.lca.no
Developer of EPD generator Phone: +47 916 50 916
LCA.no AS e-mail: post@lca.no
Dokka 6B,1671 Kråkerøy web: www.lca.no
ECO Platform web: www.eco-platform.org
ECO Portal web: ECO Portal
14 / 14
