Environmental product declaration
in accordance with ISO 14025 and EN 15804+A2
Norgips Light Board 13
Owner of the declaration: Program operator:
Norgips Norge AS The Norwegian EPD Foundation
Product: Declaration number:
Norgips Light Board 13 NEPD-8322-7979-EN
Declared unit: Registration number:
1 m2 NEPD-8322-7979-EN
This declaration is based on Product Category Rules: Issue date:
CEN Standard EN 15804:2012+A2:2019 serves as core 03.12.2024
PCR
Valid to:
The Norwegian EPD Foundation NPCR 010:2022 Part B for building boards
03.12.2029
EPD software:
LCAno EPD generator ID: 656825
1 / 12
General information
Product Owner of the declaration:
Norgips Light Board 13 Norgips Norge AS
Contact person: Trond Even Fagerli
Phone: +47 33 78 48 00
e-mail: ordre@norgips.com
Program operator: Manufacturer:
The Norwegian EPD Foundation Norgips Norge AS
Post Box 5250 Majorstuen, 0303 Oslo, Norway
Phone: +47 977 22 020
web: www.epd-norge.no
Declaration number: Place of production:
Norgips Norge AS
NEPD-8322-7979-EN
Svelvikveien 625
3060 SVELVIK, Norway
This declaration is based on Product Category Rules: Management system:
CEN Standard EN 15804:2012+A2:2019 serves as core PCR
NPCR 010:2022 Part B for building boards
Statement of liability: Organisation no:
The owner of the declaration shall be liable for the underlying 986 034 757
information and evidence. EPD Norway shall not be liable with respect
to manufacturer information, life cycle assessment data and
evidences.​
Declared unit: Issue date:
1 m2 Norgips Light Board 13 03.12.2024
Declared unit with option: Valid to:
A1-A3,A4,A5,C1,C2,C3,C4,D 03.12.2029
Year of study:
2022
Functional unit: Comparability:
1 m2 covering surface of installed building board with a specific EPD of construction products may not be comparable if they not
function, from cradle-to-grave, with activities comply with EN 15804 and seen in a building context.
needed for a study period of 60 years for the building.
General information on verification of EPD from EPD tools: Development and verification of EPD:
Independent verification of data, other environmental information The declaration is created using EPD tool lca.tools ver EPD2022.03,
and the declaration according to ISO 14025:2010, § 8.1.3 and § 8.1.4. developed by LCA.no. The EPD tool is integrated in the company's
Verification of each EPD is made according to EPD-Norway’s management system, and has been approved by EPD Norway.
guidelines for verification and approval requiring that tools are i) NEPDT96 Knauf
integrated into the company's environmental management system, ii)
the procedures for use of the EPD tool are approved by EPD-Norway, Developer of EPD: Trond Even Fagerli
and iii) the process is reviewed annually by an independent third
Reviewer of company-specific input data and EPD:​ Øystein Edland
party verifier. See Appendix G of EPD-Norway's General Programme
Instructions for further information on EPD tools
Verification of EPD tool: Approved:
Independent third party verification of the EPD tool, background data
and test-EPD in accordance with EPDNorway's procedures and
guidelines for verification and approval of EPD tools.
Håkon Hauan, CEO EPD-Norge
Third party verifier:
Elisabet Amat, GREENIZE projects
(no signature required)
2 / 12
Product
Product description:
Norgips Light Board 13 is a gypsum board composed of a plaster core encased in and firmly bonded to paper liners. The front and back paper
liners are overlapped and glued together on the backside of the board. The product is particularly suitable for the cladding of internal walls,
ceilings and partitions in all types of buildings. The long sides of the board have tapered edges, the short sides are cut. Norgips Light Board 13 has
a weight of only 7 kg/m².
It is produced with 100% renewable electric energy and liquefied natural gas (LNG)
Product specification
Norgips Light Board 13 gypsum board is produced in various widths and lengths, but with the same thickness. Therefore there are no variations
of the product per square meter.
Materials kg %
Additives 0,13 1,83
Adhesive 0,00 0,04
Chemical 0,04 0,50
Gypsum 4,39 62,73
Recycled cardboard 0,39 5,57
Recycled gypsum 1,10 15,72
Water 0,95 13,60
Total 7,00 100,00
Packaging kg %
Packaging - Cardboard 0,05 94,08
Packaging - Plastic 0,00 5,92
Total incl. packaging 7,05 100,00
Technical data:
More product information is available on www.norgips.no/www.norgips.se
Produced according to: Weight: Thickness: Reaction to fire:
EN 520 - Gypsum plasterboards 7 kg/m2 12,5 mm A2-s1,d0
Market:
Norway and Sweden
Reference service life, product
60 years
Reference service life, building or construction works
60 years
LCA: Calculation rules
Declared unit:
1 m2 Norgips Light Board 13
Cut-off criteria:
All major raw materials and all the essential energy is included. The production processes for raw materials and energy flows with very small
amounts (less than 1%) are not included when specific information are missing. These cut-off criteria do not apply for hazardous materials and
substances.
Allocation:
The allocation is made in accordance with the provisions of EN 15804. Incoming energy and water and waste production in-house is allocated
equally among all products through mass allocation. Effects of primary production of recycled materials is allocated to the main product in which
the material was used. The recycling process and transportation of the material is allocated to this analysis.
Data quality:
Specific data for the product composition are provided by the manufacturer. The data represent the production of the declared product and were
collected for EPD development in the year of study. Background data is based on EPDs according to EN 15804 and different LCA databases. The
data quality of the raw materials in A1 is presented in the table below.
3 / 12
Materials Source Data quality Year
Additives ecoinvent 3.6 Client Specific 2019
Additives ecoinvent 3.6 Database 2019
Adhesive ecoinvent 3.6 Database 2019
Chemical ecoinvent 3.6 Database 2019
Gypsum Supplier Supplier specific 2019
Packaging - Cardboard ecoinvent 3.6 Database 2019
Packaging - Plastic ecoinvent 3.6 Database 2019
Recycled cardboard S-P-08304 EPD 2021
Supplier
Recycled gypsum Supplier/ecoinvent 3.6 2019
specific/database
Water Treteknisk Specific 2021
4 / 12
System boundaries (X=included, MND=module not declared, MNR=module not relevant)
Construction Beyond the system
Product stage Use stage End of life stage
installation stage boundaries
A1 A2 A3 A4 A5 B1 B2 B3 B4 B5 B6 B7 C1 C2 C3 C4 D
X X X X X MND MND MND MND MND MND MND X X X X X
System boundary:
Flow chart for the life cycle (A1-A5 and C1-C4) with system boundaries are shown in the figure below. Modul D is also declared outside the life
cycle with material and energy substitution from net recovery and is further explained in the scenarios.
Additional technical information:
The calcined gypsum is transferred to the mixer where water and additives are added. The slurry is distributed to a plasterboard liner where the
edges are folded and a new layer of plasterboard liner is glued on to form a sandwich. The board line is continuous transferred along the
production line, cut to suitable lengths and dried in a kiln. The dried boards are cut to the correct lengths and stacked in pallets.
waR slairetam tropsnarT gnirutcafunaM tropsnarT ylbmessA e​sU ecnanetniaM riapeR tnemecalpeR tnemhsibrufeR lanoitarepO ygrene esu lanoitarepO esu retaw -eD noitcurtsnoc noitilomed tropsnarT etsaW gnissecorp lasopsiD -yrevoceR-esueR laitnetop-gnilcyceR
5 / 12
LCA: Scenarios and additional technical information
The following information describe the scenarios in the different modules of the EPD.
Capacity utilisation Value
Transport from production place to user (A4) Distance (km) Fuel/Energy Consumption Unit
(incl. return) % (Liter/tonne)
Train, Electrical (kgkm) - Norway 42,0 % 90 0,051 kWh/tkm 4,59
Truck, Biogas, 80.2% Capacity Utilisation, Class50,
80,2 % 150 0,026 l/tkm 3,90
EURO 6 (km)
Truck, Diesel, 69.2% Capacity Utilisation, Class50,
69,2 % 60 0,012 l/tkm 0,72
EURO 6 (km)
Assembly (A5) Unit Value
Material loss from installation (percent) Units/DU 0,05
Electricity, Norway (kWh) kWh/DU 0,00
Waste, packaging, plastic film (LDPE), to average
kg 0,00
treatment (kg)
Waste, packaging, folding chipboard, to average
kg 0,05
treatment (kg)
De-construction demolition (C1) Unit Value
Default scenario from PCR - demolition and
kg/DU 7,00
landfill
Electricity, Norway (kWh) kWh 0,00
Capacity utilisation Value
Transport to waste processing (C2) Distance (km) Fuel/Energy Consumption Unit
(incl. return) % (Liter/tonne)
Truck, over 32 tonnes, EURO 6 (kgkm) - Europe 53,3 % 50 0,023 l/tkm 1,15
Disposal (C4) Unit Value
Landfilling of gypsum kg 7,00
Benefits and loads beyond the system
Unit Value
boundaries (D)
Substitution of electricity, in Norway (MJ) MJ 0,00
Substitution of thermal energy, district heating, in
MJ 0,05
Norway (MJ)
6 / 12
LCA: Results
The LCA results are presented below for the declared unit defined on page 2 of the EPD document.
Environmental impact
Indicator Unit A1-A3 A4 A5 C1 C2 C3 C4 D
GWP-total kg CO2 -eq 1,14E+00 6,54E-02 1,87E-01 5,72E-05 3,07E-02 4,42E-01 5,75E-02 -2,72E-04
GWP-fossil kg CO2 -eq 1,74E+00 5,90E-02 1,03E-01 5,55E-05 3,07E-02 0,00E+00 5,74E-02 -2,63E-04
GWP-biogenic kg CO2 -eq -5,99E-01 6,43E-03 8,38E-02 1,53E-06 1,32E-05 4,42E-01 6,70E-05 -5,43E-07
GWP-luluc kg CO2 -eq 2,82E-03 5,69E-05 1,49E-04 2,29E-07 9,35E-06 0,00E+00 1,41E-05 -9,06E-06
ODP kg CFC11 -eq 2,20E-07 1,25E-08 1,54E-08 4,00E-12 7,40E-09 0,00E+00 2,17E-08 -1,92E-05
AP mol H+ -eq 6,13E-03 3,52E-04 3,64E-04 4,33E-07 9,89E-05 0,00E+00 5,11E-04 -2,17E-06
EP-FreshWater kg P -eq 6,42E-05 1,53E-06 3,06E-06 3,99E-09 2,44E-07 0,00E+00 6,51E-07 -2,34E-08
EP-Marine kg N -eq 1,86E-03 8,89E-05 1,07E-04 4,76E-08 2,16E-05 0,00E+00 1,90E-04 -7,08E-07
EP-Terrestial mol N -eq 1,81E-02 9,92E-04 1,07E-03 6,20E-07 2,41E-04 0,00E+00 2,09E-03 -7,66E-06
POCP kg NMVOC -eq 3,70E-03 3,81E-04 2,65E-04 1,67E-07 9,48E-05 0,00E+00 6,00E-04 -2,11E-06
ADP-minerals&metals1 kg Sb-eq 1,43E-05 2,58E-06 1,06E-06 4,14E-09 5,47E-07 0,00E+00 5,17E-07 -2,62E-09
ADP-fossil1 MJ 2,77E+01 1,02E+00 1,68E+00 7,57E-04 4,99E-01 0,00E+00 1,58E+00 -3,76E-03
WDP1 m3 4,81E+01 3,80E+00 3,06E+00 1,32E-01 3,82E-01 0,00E+00 9,75E+00 -4,68E-02
GWP-total = Global Warming Potential total; GWP-fossil = Global Warming Potential fossil fuels; GWP-biogenic = Global Warming Potential biogenic; GWP-luluc =
Global Warming Potential land use and land use change; ODP = Depletion potential of the stratospheric ozone layer; AP = Acidification potential, Accumulated
Exceedance; EP-freshwater = Eutrophication potential, fraction of nutrients reaching freshwater end compartment: EP-marine = Eutrophication potential, fraction of
nutrients reaching marine end compartment; EP-terrestrial = Eutrophication potential, Accumulated Exceedance; POCP = Formation potential of tropospheric ozone;
ADP-minerals&metals = Abiotic depletion potential for non-fossil resources; ADP-fossil = Abiotic depletion for fossil resources potential; WDP = Water (user)
deprivation potential, deprivation-weighted water consumption
"Reading example: 9,0 E-03 = 9,0*10-3 = 0,009"
*INA Indicator Not Assessed
1. The results of this environmental impact indicator shall be used with care as the uncertainties on these results are high or as there is limited experienced with the
indicator
Remarks to environmental impacts
7 / 12
Additional environmental impact indicators
Indicator Unit A1-A3 A4 A5 C1 C2 C3 C4 D
PM Disease incidence 3,11E-08 1,10E-08 3,63E-09 3,00E-12 2,82E-09 0,00E+00 1,09E-08 -1,31E-10
IRP2 kgBq U235 -eq 3,31E-02 4,21E-03 2,98E-03 1,37E-05 2,18E-03 0,00E+00 7,21E-03 -2,40E-05
ETP-fw1 CTUe 1,29E+01 1,26E+00 8,21E-01 3,45E-03 3,65E-01 0,00E+00 8,62E-01 -2,04E-02
HTP-c1 CTUh 4,21E-10 0,00E+00 2,10E-11 0,00E+00 0,00E+00 0,00E+00 3,50E-11 0,00E+00
HTP-nc1 CTUh 1,55E-08 2,12E-09 9,56E-10 4,00E-12 3,53E-10 0,00E+00 6,23E-10 -1,90E-11
SQP1 dimensionless 8,28E+00 2,45E+00 1,01E+00 3,81E-04 5,72E-01 0,00E+00 6,08E+00 -2,51E-02
PM = Particulate Matter emissions; IRP = Ionizing radiation – human health; ETP-fw = Eco toxicity – freshwater; HTP-c = Human toxicity – cancer effects; HTP-nc =
Human toxicity – non cancer effects; SQP = Potential Soil Quality Index (dimensionless)
"Reading example: 9,0 E-03 = 9,0*10-3 = 0,009"
*INA Indicator Not Assessed
1. The results of this environmental impact indicator shall be used with care as the uncertainties on these results are high or as there is limited experienced with the
indicator
2. This impact category deals mainly with the eventual impact of low dose ionizing radiation on human health of the nuclear fuel cycle. It does not consider effects due
to possible nuclear accidents, occupational exposure nor due to radioactive waste disposal in underground facilities. Potential ionizing radiation from the soil, from
radon and from some construction materials is also not measured by this indicator.
8 / 12
Resource use
Indicator Unit A1-A3 A4 A5 C1 C2 C3 C4 D
PERE MJ 4,16E+00 2,92E-01 2,03E-01 9,81E-03 6,27E-03 0,00E+00 5,66E-02 -2,32E-02
PERM MJ 3,95E-01 0,00E+00 -1,22E-01 0,00E+00 0,00E+00 -1,47E-04 0,00E+00 0,00E+00
PERT MJ 4,55E+00 2,92E-01 8,08E-02 9,81E-03 6,27E-03 -1,47E-04 5,66E-02 -2,32E-02
PENRE MJ 2,72E+01 9,84E-01 1,65E+00 7,58E-04 4,99E-01 0,00E+00 1,58E+00 -3,76E-03
PENRM MJ 1,65E+00 0,00E+00 -1,33E-01 0,00E+00 0,00E+00 -6,09E-01 0,00E+00 0,00E+00
PENRT MJ 2,89E+01 9,84E-01 1,52E+00 7,58E-04 4,99E-01 -6,09E-01 1,58E+00 -3,76E-03
SM kg 5,93E+00 0,00E+00 2,96E-01 0,00E+00 0,00E+00 0,00E+00 0,00E+00 0,00E+00
RSF MJ 3,42E-02 1,07E-03 1,80E-03 7,70E-06 2,19E-04 0,00E+00 1,17E-03 -4,07E-06
NRSF MJ 1,44E-02 0,00E+00 1,14E-03 1,92E-05 7,35E-04 0,00E+00 2,53E-03 -1,38E-03
FW m3 5,02E-02 4,80E-03 2,74E-03 7,32E-05 5,67E-05 0,00E+00 1,94E-03 -2,80E-05
PERE = Use of renewable primary energy excluding renewable primary energy resources used as raw materials; PERM = Use of renewable primary energy resources used
as raw materials; PERT = Total use of renewable primary energy resources; PENRE = Use of non renewable primary energy excluding non-renewable primary energy
resources used as raw materials; PENRM = Use of non renewable primary energy resources used as raw materials; PENRT = Total use of non renewable primary energy
resources; SM = Use of secondary materials; RSF = Use of renewable secondary fuels; NRSF = Use of non-renewable secondary fuels; FW = Net use of fresh water
"Reading example: 9,0 E-03 = 9,0*10-3 = 0,009"
*INA Indicator Not Assessed
9 / 12
End of life - Waste
Indicator Unit A1-A3 A4 A5 C1 C2 C3 C4 D
HWD kg 3,95E-03 3,86E-04 2,21E-04 4,86E-07 2,73E-05 0,00E+00 0,00E+00 -1,77E-07
NHWD kg 2,04E-01 1,96E-01 4,42E-01 5,83E-05 4,33E-02 0,00E+00 7,00E+00 -8,88E-05
RWD kg 4,70E-05 5,82E-06 3,77E-06 6,78E-09 3,41E-06 0,00E+00 0,00E+00 -1,97E-08
HWD = Hazardous waste disposed; NHWD = Non-hazardous waste disposed; RWD = Radioactive waste disposed
"Reading example: 9,0 E-03 = 9,0*10-3 = 0,009"
*INA Indicator Not Assessed
End of life - Output flow
Indicator Unit A1-A3 A4 A5 C1 C2 C3 C4 D
CRU kg 0,00E+00 0,00E+00 0,00E+00 0,00E+00 0,00E+00 0,00E+00 0,00E+00 0,00E+00
MFR kg 3,64E-02 0,00E+00 5,22E-02 0,00E+00 0,00E+00 0,00E+00 0,00E+00 0,00E+00
MER kg 4,81E-02 0,00E+00 6,07E-03 0,00E+00 0,00E+00 0,00E+00 0,00E+00 0,00E+00
EEE MJ 3,36E-02 0,00E+00 4,68E-03 0,00E+00 0,00E+00 0,00E+00 0,00E+00 0,00E+00
EET MJ 5,08E-01 0,00E+00 7,08E-02 0,00E+00 0,00E+00 0,00E+00 0,00E+00 0,00E+00
CRU = Components for re-use; MFR = Materials for recycling; MER = Materials for energy recovery; EEE = Exported energy electrical; EET = Exported energy thermal
"Reading example: 9,0 E-03 = 9,0*10-3 = 0,009"
*INA Indicator Not Assessed
Biogenic Carbon Content
Indicator Unit At the factory gate
Biogenic carbon content in product kg C 1,30E-01
Biogenic carbon content in accompanying packaging kg C 2,47E-02
Note: 1 kg biogenic carbon is equivalent to 44/12 kg CO2
10 / 12
Additional requirements
Greenhouse gas emissions from the use of electricity in the manufacturing phase
National production mix from import, low voltage (production of transmission lines, in addition to direct emissions and losses in grid) of applied
electricity for the manufacturing process (A3).
Electricity mix Source Amount Unit
Renewable electricity Norgips, based on 100% hydro power, with Guarantee of Origin from Glitre Energi Strøm AS 2022 Modified ecoinvent g CO2-
9,66
(kWh) 3.6 eq/kWh
Dangerous substances
The product contains no substances given by the REACH Candidate list.
Indoor environment
Emissions to indoor air are tested by RISE in 2020 and evaluated according to EN 16516.
The test are performed according to ISO 16000-9 and the calculation and reporting of TVOC according to EN 16516.
The test results of Norgips Standard 12.5 mm Typ A are in compliance with the emission requirements of Sintef Miljøcertifikat.
The emission results can be compared to different Emission Labelling Systems.
Additional Environmental Information
Additional environmental impact indicators required in NPCR Part A for construction products
Indicator Unit A1-A3 A4 A5 C1 C2 C3 C4 D
GWPIOBC kg CO2 -eq 1,71E+00 6,54E-02 1,04E-01 5,71E-05 3,07E-02 0,00E+00 5,74E-02 -2,69E-04
GWP-IOBC: Global warming potential calculated according to the principle of instantaneous oxidation. In order to increase the transparency of biogenic carbon​
contribution to climate impact, the indicator GWP-IOBC is required as it declares climate impacts calculated according to the principle of instantaneous oxidation.​
GWP-IOBC is also referred to as GWP-GHG in context to Swedish public procurement legislation.
11 / 12
Bibliography
ISO 14025:2010 Environmental labels and declarations - Type III environmental declarations - Principles and procedures.
ISO 14044:2006 Environmental management - Life cycle assessment - Requirements and guidelines.
EN 15804:2012+A2:2019 Environmental product declaration - Core rules for the product category of construction products.
ISO 21930:2017 Sustainability in buildings and civil engineering works - Core rules for environmental product declarations of construction
products.
ecoinvent v3, Allocation, cut-off by classification, Swiss Centre of Life Cycle Inventories.
Iversen et al., (2021) eEPD v2021.09 Background information for EPD generator tool system verification, LCA.no Report number: 07.21
Vold, M. et al. (2022) EPD generator for Building boards
Background information for EPD generator application and LCA data, LCA.no report number 05.22
NPCR Part A: Construction products and services. Ver. 2.0. April 2021, EPD-Norge.
NPCR 010 Part B for Building Boards. Ver. 4.0, March 2022, EPD-Norge.
Program operator and publisher Phone: +47 977 22 020
The Norwegian EPD Foundation e-mail: post@epd-norge.no
Post Box 5250 Majorstuen, 0303 Oslo, Norway web: www.epd-norge.no
Owner of the declaration: Phone: +47 33 78 48 00
Norgips Norge AS e-mail: ordre@norgips.com
Svelvikveien 625, 3060 SVELVIK, Norway web: www.norgips.no
Author of the Life Cycle Assessment Phone: +47 916 50 916
LCA.no AS e-mail: post@lca.no
Dokka 6A, 1671 Kråkerøy, Norway web: www.lca.no
Developer of EPD generator Phone: +47 916 50 916
LCA.no AS e-mail: post@lca.no
Dokka 6A, 1671 Kråkerøy, Norway web: www.lca.no
ECO Platform web: www.eco-platform.org
ECO Portal web: ECO Portal
12 / 12
