Environmental product declaration
in accordance with ISO 14025 and EN 15804+A2
Envistar Top 17 with counter-flow heat exchanger and controls
Owner of the declaration: Program operator:
IV Produkt AB The Norwegian EPD Foundation
Product: Declaration number:
Envistar Top 17 with counter-flow heat exchanger and
controls NEPD-9368-8955
Declared unit: Registration number:
1 pcs
NEPD-9368-8955
This declaration is based on Product Category Rules:
Issue date: 10.03.2025
CEN Standard EN 15804:2012+A2:2019 serves as core
The Norwegian EPD Foundation PCR Valid to: 10.03.2030
NPCR 030:2021 Part B for ventilation components
EPD software:
LCAno EPD generator ID: 805232
1 / 13
General information
Product Owner of the declaration:
Envistar Top 17 with counter-flow heat exchanger and controls IV Produkt AB
Contact person:
Phone: + 46 70 758800
e-mail: info@ivprodukt.se
Program operator: Manufacturer:
The Norwegian EPD Foundation IV Produkt AB
Post Box 5250 Majorstuen, 0303 Oslo, Norway
Phone: +47 977 22 020
web: www.epd-norge.no
Declaration number: Place of production:
IV Produkt AB
NEPD-9368-8955
Sjöuddevägen 7
352 46 Växjö, Sweden
This declaration is based on Product Category Rules: Management system:
CEN Standard EN 15804:2012+A2:2019 serves as core PCR ISO 14001 and 9001
NPCR 030:2021 Part B for ventilation components
Statement of liability: Organisation no:
The owner of the declaration shall be liable for the underlying 556129-1559
information and evidence. EPD Norway shall not be liable with respect
to manufacturer information, life cycle assessment data and
evidences.​
Declared unit: Issue date:
1 pcs Envistar Top 17 with counter-flow heat exchanger and controls 10.03.2025
Declared unit with option: Valid to:
A1-A3,A4,C1,C2,C3,C4,D 10.03.2030
Year of study:
2023
Functional unit: Comparability:
N/A EPDs of construction products may not be comparable if they do not
comply with EN 15804 and are not seen in a building context.
General information on verification of EPD from EPD tools: Development and verification of EPD:
Independent verification of data, other environmental information The declaration is created using EPD tool lca.tools ver EPD2022.03,
and the declaration according to ISO 14025:2010, § 8.1.3 and § 8.1.4. developed by LCA.no. The EPD tool is integrated in the company's
Verification of each EPD is made according to EPD-Norway’s management system and has been approved by EPD Norway.
guidelines for verification and approval requiring that tools are i) NEPDT144
integrated into the company's environmental management system, ii)
the procedures for use of the EPD tool are approved by EPD-Norway, Developer of EPD: Linnea Schindelar
and iii) the process is reviewed annually by an independent third
Reviewer of company-specific input data and EPD:​ Axel bergstrand
party verifier. See Appendix G of EPD-Norway's General Programme
Instructions for further information on EPD tools
Verification of EPD tool: Approved:
Independent third party verification of the EPD tool, background data
and test-EPD in accordance with EPDNorway's procedures and
guidelines for verification and approval of EPD tools.
Third party verifier:
Alexander Borg, Asplan Viak AS
(no signature required)
2 / 13
Product
Product description:
Air Handling Unit (AHU) for non residential building.
Product specification
Envistar Top air handling unit for non residential buildings.
Bi-directional including counter-flow heat exchanger and integrated controls, damper and LPHW coil.
Materials kg %
Adhesive 2,34 0,28
Aluminium foil, with plastic 0,018 0,0022
Electronic - Unspecified 6,16 0,75
Electronic - Wire 1,51 0,18
Filter, plastic based 3,80 0,46
Glass fibre reinforced plastic,
18,23 2,22
polyamide
Insulation 32,18 3,93
Motor 13,56 1,65
Plastic - Polyamide 0,16 0,019
Plastic - Polyethylene (HDPE) 0,060 0,0073
Plastic - Polystyrene (PS) 0,085 0,010
Rubber, synthetic 0,041 0,0050
Steel and rubber 1,45 0,17
Ventilation components 27,12 3,31
Metal 2,38 0,29
Metal - Aluminium 166,43 20,33
Metal - Brass 0,41 0,050
Metal - Steel 14,95 1,82
Metal - Steel with aluzinc coating 527,21 64,40
Plastic - Polyethylene terephthalate
0,47 0,058
(PET)
Plastic - Acrylonitrile butadiene
0,0060 0,00073
styrene (ABS)
Total 818,65 100,00
Packaging kg %
Packaging - PET Film 3,50 100,00
Total incl. packaging 822,15 100,00
Technical data:
According to printout from IVP Designer (selection program).
Market:
Europe
Reference service life, product
25 years
Reference service life, building or construction works
N/A
LCA: Calculation rules
Declared unit:
1 pcs Envistar Top 17 with counter-flow heat exchanger and controls
Cut-off criteria:
All major raw materials and all the essential energy is included. The production processes for raw materials and energy flows with very small
amounts (less than 1%) are not included. These cut-off criteria do not​ apply for hazardous materials and substances.
Allocation:
The allocation is made in accordance with the provisions of EN 15804. Energy, water and waste production in-house is allocated equally among all
products through mass allocation. Effects of primary production of recycled materials is allocated to the main product in which the material was
used. The recycling process and transportation of the material is allocated to this analysis.
Data quality:
3 / 13
Specific data for the product composition are provided by the manufacturer. The data represent the production of the declared product and were
collected for EPD development in the year of study. Background data is based on EPDs according to EN 15804 and different LCA databases. The
data quality of the raw materials in A1 is presented in the table below.
Materials Source Data quality Year
Adhesive ecoinvent 3.6 Database 2019
Aluminium foil, with plastic ecoinvent 3.6 Database 2019
Electronic - Unspecified ecoinvent 3.6 Database 2019
Electronic - Wire ecoinvent 3.6 Database 2019
Filter, plastic based S-P-03432 EPD 2022
Glass fibre reinforced plastic, polyamide ecoinvent 3.6 Database 2019
Insulation ecoinvent 3.6 Database 2019
Metal ecoinvent 3.6 Database 2019
Metal - Aluminium ecoinvent 3.6 Database 2019
Metal - Aluminium Modified ecoinvent 3.6 Database 2019
Metal - Brass ecoinvent 3.6 Database 2019
Metal - Steel ecoinvent 3.6 Database 2019
Metal - Steel with aluzinc coating Modified ecoinvent 3.6 Database 2019
Motor ecoinvent 3.6 Database 2019
Packaging - PET Film Ecoinvent 3.6 Database 2019
Plastic - Acrylonitrile butadiene styrene (ABS) ecoinvent 3.6 Database 2019
Plastic - Polyamide ecoinvent 3.6 Database 2019
Plastic - Polyethylene (HDPE) ecoinvent 3.6 Database 2019
Plastic - Polyethylene terephthalate (PET) ecoinvent 3.6 Database 2019
Plastic - Polystyrene (PS) ecoinvent 3.6 Database 2019
Rubber, synthetic ecoinvent 3.6 Database 2019
Steel and rubber ecoinvent 3.6 Database 2019
Ventilation components ecoinvent 3.6 Database 2019
4 / 13
System boundaries (X=included, MND=module not declared, MNR=module not relevant)
Construction Beyond the system
Product stage Use stage End of life stage
installation stage boundaries
A1 A2 A3 A4 A5 B1 B2 B3 B4 B5 B6 B7 C1 C2 C3 C4 D
X X X X MND MND MND MND MND MND MND MND X X X X X
System boundary:
Additional technical information:
The unit is made up of frameworks in aluminium profiles. Panels and hatches are in double sheet construction of aluminium/zinc-treated steel
sheet with protective coating (ALC) that meets the requirements for corrosion class C4 according to SS-EN ISO 12944-2.
Development and manufacture of our products takes place with the help of our environmental and quality management system certified according
to ISO 14001 and ISO 9001.
Units delivered are CE-marked.
IV Produkt AB's unit series are certified by Eurovent as standard.
Complete project specific technical documentation is generated using our selection software, IVP Designer.
Please refer to our website www.ivprodukt.se for more information.
waR slairetam tropsnarT gnirutcafunaM tropsnarT ylbmessA e​sU ecnanetniaM riapeR tnemecalpeR tnemhsibrufeR lanoitarepO ygrene esu lanoitarepO esu retaw -eD noitcurtsnoc noitilomed tropsnarT etsaW gnissecorp lasopsiD -yrevoceR-esueR laitnetop-gnilcyceR
5 / 13
LCA: Scenarios and additional technical information
The following information describe the scenarios in the different modules of the EPD.
Module A4 = A generic transportation distance (EURO6 truck) of 378 km is declared. True transportation distance can be provided in project
specific EPD.
Module A5 = Not declared.
Module C1 = The de-installation of the air handling unit (AHU) is carried out manually, with the assistance of electrical tools. The energy
consumption of portable electrical devices (e.g., drills) is typically low, falling below the 1% cut-off criterion, and is therefore disregarded.
Module C2 = A generic transportation distance (EURO6 truck) of 80 km is declared. True transportation distance can be provided in project
specific EPD.
Modules C3 and C4 = Waste treatment of the product follows the default values provided in EN 15804:2012+A2:2019 and EN 50693, Product
Category Rules for life cycle assessments of electronic and electrical products and systems, table G.4. This table specified how different types of raw
materials used in A1 will likely be treated during the end-of-life of the product. Waste treatments in C3 include material recycling and incineration
with and without energy recovery and fly ash extraction. Disposal in C4 consist of landfilling of different waste fractions and of ashes.
Module D = The recyclability of metals, plastics, and electronic components allows the producers a credit for the net scrap that is produced at the
end of a product’s life. The benefits from recycling of net scrap are described in formula from EN 15804:2012+A2:2019. Substitution of heat and
electricity generated by the incineration with energy recovery of plastic insulation and other parts is also calculated in module D.
Capacity utilisation Value
Transport from production place to user (A4) Distance (km) Fuel/Energy Consumption Unit
(incl. return) % (Liter/tonne)
Truck, 16-32 tonnes, EURO 6 (km) 36,7 % 378 0,043 l/tkm 16,25
Truck, over 32 tonnes, EURO 6 (km) 53,3 % 378 0,023 l/tkm 8,69
Capacity utilisation Value
Transport to waste processing (C2) Distance (km) Fuel/Energy Consumption Unit
(incl. return) % (Liter/tonne)
Truck, 16-32 tonnes, EURO 6 (km) 36,7 % 80 0,043 l/tkm 3,44
Waste processing (C3) Unit Value
Waste treatment per kg Non-hazardous waste,
kg 18,23
incineration with fly ash extraction (kg)
Waste treatment per kg electronics scrap from
PWB, with components, recycling of metals C3 kg 3,082
(kg)
Waste treatment per kg wire plastic, municipal
kg 0,24
incineration (kg)
Materials to recycling (kg) kg 683,60
Waste treatment per kg Polypropylene (PP),
kg 0,23
incineration (kg)
Aluminium to recycling (kg) kg 0,011
Waste treatment per kg Polyethylene
terephthalate (PET), incineration with fly ash kg 0,042
extraction (kg)
Waste treatment per kg Hazardous waste,
kg 38,33
incineration (kg)
Waste treatment per kg Rubber, municipal
kg 0,041
incineration with fly ash extraction (kg)
Waste treatment per kg used PWB, shredding and
kg 6,16
separation - C3 (kg)
Waste treatment per kg bulk waste, excluding
kg 13,56
reinforcement, sorting plant (kg)
Waste treatment per kg Plastics, from incineration
kg 0,083
(kg)
Waste treatment per kg Polyethylene, PE,
kg 0,060
incineration with fly ash extraction (kg)
Waste treatment of plastic mixture, incineration
kg 0,36
with energy recovery and fly ash extraction (kg)
6 / 13
Disposal (C4) Unit Value
Waste, copper, to landfill (kg) kg 0,31
Waste, aluminium, to landfill (kg) kg 11,74
Landfilling of ashes from incineration of Plastics,
kg 0,014
process per kg ashes and residues (kg)
Waste, scrap steel, to landfill (kg) kg 58,13
Landfilling of ashes from incineration of Non-
hazardous waste process per kg ashes and kg 4,32
residues (kg)
Waste, plastic, mixture, to landfill (kg) kg 0,97
Landfilling of ashes from incineration of
Polyethylene (PE), process per kg ashes and kg 0,0021
residues (kg)
Landfilling of ashes from incineration per kg wire
kg 0,037
plastic, from municipal incineration - RoW
Landfilling of hazardous waste (kg) kg 3,082
Landfilling of ashes from incineration of
Polypropylene (PP), process per kg ashes and kg 0,0070
residues (kg)
Waste treatment per kg Brass slag, to landfill,
kg 0,041
residual material landfill (kg)
Landfilling of ashes from incineration per kg
kg 7,24
Hazardous waste, from incineration (kg)
Landfilling of ashes from incineration of
Polyethylene terephthalate (PET), process per kg kg 0,00095
ashes and residues (kg)
Landfilling of ashes from incineration of Rubber,
kg 0,0021
municipal incineration with fly ash extraction (kg)
Benefits and loads beyond the system
Unit Value
boundaries (D)
Substitution of primary Brass with net scrap (kg) kg 0,37
Substitution of electricity (MJ) MJ 12,35
Substitution of thermal energy, district heating
MJ 186,97
(MJ)
Substitution of primary aluminium with net scrap
kg 154,98
(kg)
Substitution of primary metals with net scrap
kg 0,90
from PWB, with components (kg)
Substitution of primary copper with net scrap (kg) kg 1,61
Substitution of primary steel with net scrap (kg) kg 298,084
7 / 13
LCA: Results
The LCA results are presented below for the declared unit defined on page 2 of the EPD document.
Environmental impact
Indicator Unit A1-A3 A4 C1 C2 C3 C4 D
GWP-total kg CO2 -eq 4,34E+03 3,44E+01 0,00E+00 1,07E+01 1,32E+02 4,42E+00 -1,79E+03
GWP-fossil kg CO2 -eq 4,29E+03 3,44E+01 0,00E+00 1,07E+01 1,32E+02 4,41E+00 -1,76E+03
GWP-biogenic kg CO2 -eq 2,93E+01 1,45E-02 0,00E+00 4,45E-03 2,16E-01 3,10E-03 -6,68E+00
GWP-luluc kg CO2 -eq 2,02E+01 1,13E-02 0,00E+00 3,82E-03 2,61E-02 6,24E-03 -2,64E+01
ODP kg CFC11 -eq 3,38E-04 8,07E-06 0,00E+00 2,43E-06 1,02E-05 3,65E-07 -7,91E-02
AP mol H+ -eq 3,77E+01 1,05E-01 0,00E+00 3,09E-02 1,37E-01 1,34E-02 -1,50E+01
EP-FreshWater kg P -eq 2,71E-01 2,74E-04 0,00E+00 8,58E-05 2,09E-03 6,57E-05 -9,68E-02
EP-Marine kg N -eq 4,81E+00 2,21E-02 0,00E+00 6,11E-03 2,93E-02 3,84E-03 -1,71E+00
EP-Terrestial mol N -eq 8,74E+01 2,47E-01 0,00E+00 6,83E-02 3,27E-01 4,21E-02 -1,92E+01
POCP kg NMVOC -eq 1,77E+01 9,60E-02 0,00E+00 2,62E-02 9,11E-02 1,33E-02 -6,80E+00
ADP-minerals&metals1 kg Sb-eq 1,22E+00 7,67E-04 0,00E+00 2,97E-04 3,29E-04 1,37E-05 -9,42E-02
ADP-fossil1 MJ 5,36E+04 5,41E+02 0,00E+00 1,62E+02 3,77E+02 3,47E+01 -2,10E+04
WDP1 m3 5,91E+05 4,63E+02 0,00E+00 1,57E+02 1,46E+03 5,04E+02 -7,73E+05
GWP-total = Global Warming Potential total; GWP-fossil = Global Warming Potential fossil fuels; GWP-biogenic = Global Warming Potential biogenic; GWP-luluc =
Global Warming Potential land use and land use change; ODP = Depletion potential of the stratospheric ozone layer; AP = Acidification potential, Accumulated
Exceedance; EP-freshwater = Eutrophication potential, fraction of nutrients reaching freshwater end compartment: EP-marine = Eutrophication potential, fraction of
nutrients reaching marine end compartment; EP-terrestrial = Eutrophication potential, Accumulated Exceedance; POCP = Formation potential of tropospheric ozone;
ADP-minerals&metals = Abiotic depletion potential for non-fossil resources; ADP-fossil = Abiotic depletion for fossil resources potential; WDP = Water (user)
deprivation potential, deprivation-weighted water consumption
"Reading example: 9,0 E-03 = 9,0*10-3 = 0,009"
*INA Indicator Not Assessed
1. The results of this environmental impact indicator shall be used with care as the uncertainties on these results are high or as there is limited experienced with the
indicator
Remarks to environmental impacts
8 / 13
Additional environmental impact indicators
Indicator Unit A1-A3 A4 C1 C2 C3 C4 D
PM Disease incidence 3,78E-04 2,68E-06 0,00E+00 6,58E-07 1,99E-06 1,77E-07 -1,32E-04
IRP2 kgBq U235 -eq 2,16E+02 2,37E+00 0,00E+00 7,10E-01 1,73E+00 1,57E-01 -7,77E+01
ETP-fw1 CTUe 1,97E+05 3,98E+02 0,00E+00 1,20E+02 1,89E+03 7,34E+03 -6,95E+04
HTP-c1 CTUh 1,70E-05 0,00E+00 0,00E+00 0,00E+00 1,37E-07 1,41E-08 -5,27E-06
HTP-nc1 CTUh 2,52E-04 4,07E-07 0,00E+00 1,32E-07 3,64E-06 6,87E-07 -2,26E-05
SQP1 dimensionless 1,51E+04 5,14E+02 0,00E+00 1,14E+02 1,47E+02 1,02E+02 -1,04E+03
PM = Particulate Matter emissions; IRP = Ionizing radiation – human health; ETP-fw = Eco toxicity – freshwater; HTP-c = Human toxicity – cancer effects; HTP-nc =
Human toxicity – non cancer effects; SQP = Potential Soil Quality Index (dimensionless)
"Reading example: 9,0 E-03 = 9,0*10-3 = 0,009"
*INA Indicator Not Assessed
1. The results of this environmental impact indicator shall be used with care as the uncertainties on these results are high or as there is limited experienced with the
indicator
2. This impact category deals mainly with the eventual impact of low dose ionizing radiation on human health of the nuclear fuel cycle. It does not consider effects due
to possible nuclear accidents, occupational exposure nor due to radioactive waste disposal in underground facilities. Potential ionizing radiation from the soil, from
radon and from some construction materials is also not measured by this indicator.
9 / 13
Resource use
Indicator Unit A1-A3 A4 C1 C2 C3 C4 D
PERE MJ 1,34E+04 7,22E+00 0,00E+00 2,32E+00 6,73E+01 5,05E+00 -6,74E+03
PERM MJ 8,23E+00 0,00E+00 0,00E+00 0,00E+00 0,00E+00 0,00E+00 0,00E+00
PERT MJ 1,34E+04 7,22E+00 0,00E+00 2,32E+00 6,73E+01 5,05E+00 -6,74E+03
PENRE MJ 5,36E+04 5,41E+02 0,00E+00 1,62E+02 3,78E+02 3,48E+01 -2,10E+04
PENRM MJ 8,80E+02 0,00E+00 0,00E+00 0,00E+00 -5,74E+02 0,00E+00 0,00E+00
PENRT MJ 5,44E+04 5,41E+02 0,00E+00 1,62E+02 -1,96E+02 3,48E+01 -2,10E+04
SM kg 3,01E+02 0,00E+00 0,00E+00 0,00E+00 1,50E-04 6,66E-02 1,01E+00
RSF MJ 8,12E+01 2,55E-01 0,00E+00 8,32E-02 1,46E+00 5,33E-02 9,31E+00
NRSF MJ 9,66E+02 8,83E-01 0,00E+00 2,97E-01 -2,96E-03 9,15E-01 3,49E+02
FW m3 1,03E+02 6,00E-02 0,00E+00 1,74E-02 3,70E-01 4,56E-02 -3,60E+01
PERE = Use of renewable primary energy excluding renewable primary energy resources used as raw materials; PERM = Use of renewable primary energy resources used
as raw materials; PERT = Total use of renewable primary energy resources; PENRE = Use of non renewable primary energy excluding non-renewable primary energy
resources used as raw materials; PENRM = Use of non renewable primary energy resources used as raw materials; PENRT = Total use of non renewable primary energy
resources; SM = Use of secondary materials; RSF = Use of renewable secondary fuels; NRSF = Use of non-renewable secondary fuels; FW = Net use of fresh water
"Reading example: 9,0 E-03 = 9,0*10-3 = 0,009"
*INA Indicator Not Assessed
10 / 13
End of life - Waste
Indicator Unit A1-A3 A4 C1 C2 C3 C4 D
HWD kg 3,15E+01 2,89E-02 0,00E+00 8,38E-03 1,56E-03 4,06E+00 3,85E+00
NHWD kg 1,27E+03 3,79E+01 0,00E+00 7,90E+00 5,86E+01 7,87E+01 -5,45E+02
RWD kg 1,95E-01 3,69E-03 0,00E+00 1,11E-03 7,81E-05 5,02E-06 -7,30E-02
HWD = Hazardous waste disposed; NHWD = Non-hazardous waste disposed; RWD = Radioactive waste disposed
"Reading example: 9,0 E-03 = 9,0*10-3 = 0,009"
*INA Indicator Not Assessed
End of life - Output flow
Indicator Unit A1-A3 A4 C1 C2 C3 C4 D
CRU kg 0,00E+00 0,00E+00 0,00E+00 0,00E+00 0,00E+00 0,00E+00 0,00E+00
MFR kg 6,29E+01 0,00E+00 0,00E+00 0,00E+00 6,84E+02 1,21E-04 -6,05E-02
MER kg 2,05E+01 0,00E+00 0,00E+00 0,00E+00 5,76E+01 3,32E-06 -7,79E-03
EEE MJ 1,21E+01 0,00E+00 0,00E+00 0,00E+00 1,52E+00 1,43E-04 -2,67E-02
EET MJ 1,83E+02 0,00E+00 0,00E+00 0,00E+00 2,31E+01 2,17E-03 -4,04E-01
CRU = Components for re-use; MFR = Materials for recycling; MER = Materials for energy recovery; EEE = Exported energy electrical; EET = Exported energy thermal
"Reading example: 9,0 E-03 = 9,0*10-3 = 0,009"
*INA Indicator Not Assessed
Biogenic Carbon Content
Indicator Unit At the factory gate
Biogenic carbon content in product kg C 0,00E+00
Biogenic carbon content in accompanying packaging kg C 0,00E+00
Note: 1 kg biogenic carbon is equivalent to 44/12 kg CO2
11 / 13
Additional requirements
Greenhouse gas emissions from the use of electricity in the manufacturing phase
National production mix from import, low voltage (production of transmission lines, in addition to direct emissions and losses in grid) of applied
electricity for the manufacturing process (A3).
Electricity mix Source Amount Unit
Electricity, Sweden (kWh) ecoinvent 3.6 54,94 g CO2-eq/kWh
Dangerous substances
The product contains no substances given by the REACH Candidate list.
Indoor environment
Additional Environmental Information
Additional environmental impact indicators required in NPCR Part A for construction products
Indicator Unit A1-A3 A4 C1 C2 C3 C4 D
GWPIOBC kg CO2 -eq 4,33E+03 3,44E+01 0,00E+00 1,07E+01 1,13E+02 4,56E+00 -1,89E+03
GWP-IOBC: Global warming potential calculated according to the principle of instantaneous oxidation. In order to increase the transparency of biogenic carbon​
contribution to climate impact, the indicator GWP-IOBC is required as it declares climate impacts calculated according to the principle of instantaneous oxidation.​
GWP-IOBC is also referred to as GWP-GHG in context to Swedish public procurement legislation.
12 / 13
Bibliography
ISO 14025:2010 Environmental labels and declarations - Type III environmental declarations - Principles and procedures.
ISO 14044:2006 Environmental management - Life cycle assessment - Requirements and guidelines.
EN 15804:2012+A2:2019 Environmental product declaration - Core rules for the product category of construction products.
ISO 21930:2017 Sustainability in buildings and civil engineering works - Core rules for environmental product declarations of construction
products.
ecoinvent v3, Allocation, cut-off by classification, Swiss Centre of Life Cycle Inventories.
Iversen et al., (2021) eEPD v2021.09 Background information for EPD generator tool system verification, LCA.no Report number: 07.21
Graafland and Iversen (2022) EPD generator for NPCR 030 Ventilation components, Background information for EPD generator application and
LCA data, LCA.no report number: 12.22
NPCR Part A: Construction products and services. Ver. 2.0. April 2021, EPD-Norge.
NPCR 030 Part B for Ventilation components, Ver. 1.0, 18.05.2021, EPD Norway.
Program operator and publisher Phone: +47 977 22 020
The Norwegian EPD Foundation e-mail: post@epd-norge.no
Post Box 5250 Majorstuen, 0303 Oslo, Norway web: www.epd-norge.no
Owner of the declaration: Phone: +46 70 758800
IV Produkt AB e-mail: info@ivprodukt.se
Sjöuddevägen 7, 352 46 Växjö, Sweden web: www.ivprodukt.se
Author of the Life Cycle Assessment Phone: +47 916 50 916
LCA.no AS e-mail: post@lca.no
Dokka 6A, 1671 Kråkerøy, Norway web: www.lca.no
Developer of EPD generator Phone: +47 916 50 916
LCA.no AS e-mail: post@lca.no
Dokka 6A, 1671 Kråkerøy, Norway web: www.lca.no
ECO Platform web: www.eco-platform.org
ECO Portal web: ECO Portal
13 / 13
