Environmental product declaration
In accordance with 14025 and EN15804+A2
Place
Owner of the declaration: Program operator:
Elektroskandia Norge AS The Norwegian EPD Foundation
Product: Declaration number:
Place
Registration number:
Declared unit:
1 pcs Issue date:
This declaration is based on Product Category Rules: Valid to:
CEN Standard EN 15804:2012+A2:2019 serves as core
EPD Software:
PCR
LCA.no EPD generator ID: 60258
IBU PCR - Part B for luminaires, lamps, and components
The Norwegian EPD Foundation for luminaires
1 / 13
General information
Product Owner of the declaration:
Place Elektroskandia Norge AS
Contact person: Pål Kristiansen
Phone: +47 97 66 22 12
e-mail: pkr@elektroskandia.no
Program operator: Manufacturer:
Post Box 5250 Majorstuen, 0303 Oslo, Norway SG Armaturen AS
The Norwegian EPD Foundation Skytterheia 25
Phone: +47 23 08 80 00 4790 Lillesand, Norway
web: post@epd-norge.no
Declaration number: Place of production:
SG Armaturen production site Odense (Denmark)
Egestubben 26
5270 Odense, Denmark
This declaration is based on Product Category Rules: Management system:
CEN Standard EN 15804:2012+A2:2019 serves as core PCR ISO 14001, ISO 9001
IBU PCR - Part B for luminaires, lamps, and components for
luminaires
Statement of liability: Organisation no:
The owner of the declaration shall be liable for the underlying 977 454 700
information and evidence. EPD Norway shall not be liable with respect
to manufacturer information, life cycle assessment data and
evidences.​
Declared unit: Issue date:
1 pcs Place
Declared unit with option: Valid to:
A1,A2,A3,A4,A5,C1,C2,C3,C4,D
Year of study:
2022
Functional unit: Comparability:
1 Place LED luminaire manufactured and installed, including waste EPD of construction products may not be comparable if they not
treatment at end-of-life. comply with EN 15804 and seen in a building context.
General information on verification of EPD from EPD tools: Development and verification of EPD:
Independent verification of data, other environmental information The declaration is created using EPD tool lca.tools ver EPD2021.09,
and the declaration according to ISO 14025:2010, § 8.1.3 and § 8.1.4. developed by LCA.no. The EPD tool is integrated in the company's
Individualthird party verification of each EPD is not required when the management system, and has been approved by EPD Norway.
EPD tool is i) integrated into the company's environmental
management system, ii) the procedures for use of the EPD tool are Developer of EPD: Pål Pedersen, Elektroskandia Norge AS
approved by EPDNorway, and iii)the proccess is reviewed annualy. See
Reviewer of company-specific input data and EPD:​ Pål Pedersen,
Appendix G of EPD-Norway's General Programme Instructions for
Elektroskandia Norge AS
further information on EPD tools.
Verification of EPD tool: Approved:
Independent third party verification of the EPD tool, background data
and test-EPD in accordance with EPDNorway's procedures and
guidelines for verification and approval of EPD tools. Approval
number: NEPDT41.
Third party verifier:
Vito D’Incognito - Take Care International
(no signature required)
2 / 13
Product
Product description:
Mast or wall-mounted (600 mm diameter) IP66 LED luminaire. Base and top made of die-cast aluminium, inner diffuser made of PMMA and outer
optics made of polycarbonate (PC). Grey or black base and top. Complete with LED driver for operation of LED light sources mounted to
component rail with internal connector/lampholder and pre-mounted with five-metre connection cable. Prepared for mounting on 60 mm or
designer mast. Safety class II.
Wattage: 28W. Luminous flux: 2510lm. Efficacy: 90 lm/W. Colour temperature: 4000K. Colour rendering: Ra>80. Housing: Die-cast aluminum.
Colour: Grey (structure 2150 sablé). Height: 291 mm. Diameter: 600 mm. EAN: 5703821168090.
The EPD also covers the following products:
EAN: 5703821168076 - Place Grey 2370lm 3000K Ra>80 DYNADIM Pr. 2 Sweden
EAN: 5703821172097 - Place Black 2370lm 3000K Ra>80 DYNADIM Pr. 2 Sweden
EAN: 5703821172110 - Place Black 2510lm 4000K Ra>80 DYNADIM Pr. 2 Sweden
EAN: 5703821172950 - Place Grey 2370lm 3000K Ra>80 Lumistep LS8
EAN: 5703821172967 - Place Grey 2510lm 4000K Ra>80 Lumistep LS8
Product specification
Materials kg %
0,02 0,25
Coating materials 0,09 1,22
Electronic - Connector 0,01 0,12
Electronic - LED chip 0,04 0,52
Electronic - LED driver 0,21 2,81
Electronic - LED plate 0,46 6,13
Electronic - Wire 0,51 6,88
Metal - Aluminium 3,40 45,53
Metal - Stainless steel 0,11 1,43
Metal - Steel 0,08 1,07
Plastic - Plexiglass (PMMA) 1,06 14,27
Plastic - Polycarbonate (PC) 1,22 16,35
Powder coating 0,14 1,84
Rubber, synthetic 0,01 0,16
Silicon products 0,11 1,41
Total 7,46
Packaging kg %
Packaging - Cardboard 0,20 72,97
Packaging - Plastic 0,07 27,03
Total incl. packaging 7,73
Technical data:
Link to the CE Declaration on our website:
https://www.sg-as.com/storage/data/130987_Place/50/130987_Place.pdf
Link to product data on our website:
https://www.sg-as.com/products/place-wall-arm/8246088228
Market:
Norway.
Reference service life, product
The declared service life of the product is 25 years.
This is estimated based on the characteristics of the product, intended application and previous knowledge/experience for that type of luminaire.
Reference service life, building or construction works
LCA: Calculation rules
Declared unit:
1 pcs Place
Cut-off criteria:
All major raw materials and all the essential energy is included. The production processes for raw materials and energy flows with very small
amounts (less than 1%) can be excluded. These cut-off criteria do not apply for hazardous materials and substances.
3 / 13
Allocation:
The allocation is made in accordance with the provisions of EN 15804. Incoming energy and water and waste production in-house is allocated
equally among all products through mass allocation. Effects of primary production of recycled materials is allocated to the main product in which
the material was used. The recycling process and transportation of the material is allocated to this analysis.
Data quality:
Specific data for the product composition are provided by the manufacturer. The data represent the production of the declared product and were
collected for EPD development in the year of study. Background data is based on EPDs according to EN 15804 and different LCA databases. The
data quality of the raw materials in A1 is presented in the table below.
Materials Source Data quality Year
Coating materials Ecoinvent 3.6 Database 2019
Electronic - Connector ecoinvent 3.6 Database 2019
Electronic - LED plate ecoinvent 3.6 Database 2019
Metal - Aluminium ecoinvent 3.6 Database 2019
Metal - Stainless steel ecoinvent 3.6 Database 2019
Metal - Steel ecoinvent 3.6 Database 2019
Packaging - Cardboard ecoinvent 3.6 Database 2019
Packaging - Plastic ecoinvent 3.6 Database 2019
Plastic - Plexiglass (PMMA) ecoinvent 3.6 Database 2019
Plastic - Polycarbonate (PC) ecoinvent 3.6 Database 2019
Powder coating Ecoinvent 3.6 Database 2019
Rubber, synthetic ecoinvent 3.6 Database 2019
Silicon products ecoinvent 3.6 Database 2019
Supplier data +
Electronic - Connector Material composition + ecoinvent 3.6 2019
database
Supplier data +
Electronic - LED driver Material composition + ecoinvent 3.6 2019
database
Supplier data +
Electronic - Wire Material composition + ecoinvent 3.6 2019
database
Metal - Aluminium Modified ecoinvent 3.6 Database 2019
Metal - Stainless steel Modified ecoinvent 3.6 Database 2019
Supplier data +
Electronic - Wire Product composition + ecoinvent 3.6 2019
database
Scientific
Electronic - LED chip Scholand et al. (2012) + Ecoinvent 3.6 literature + 2017
database
4 / 13
System boundaries (X=included, MND=module not declared, MNR=module not relevant)
Construction Beyond the system
Product stage Use stage End of life stage
installation stage boundaries
A1 A2 A3 A4 A5 B1 B2 B3 B4 B5 B6 B7 C1 C2 C3 C4 D
X X X X X MND MND MND MND MND MND MND X X X X X
System boundary:
Additional technical information:
Link to the user manual on our website, for proper use of the product:
https://www.sg-as.com/storage/data/130987_Place/20/130987_Place_User%20Manual.pdf
waR slairetam tropsnarT gnirutcafunaM tropsnarT ylbmessA e​sU ecnanetniaM riapeR tnemecalpeR tnemhsibrufeR lanoitarepO ygrene esu lanoitarepO esu retaw -eD noitcurtsnoc noitilomed tropsnarT etsaW gnissecorp lasopsiD -yrevoceR-esueR laitnetop-gnilcyceR
5 / 13
LCA: Scenarios and additional technical information
The following information describe the scenarios in the different modules of the EPD.
Module A4 = Transportation from production site in Odense, Denmark to Elektroskandia, Langhus, Norway 600 km + 300 km for Norwegian
market.
Module A5 = Installation is performed in Norway and done by manual labor, with the use of electrical machines, that fall under the cut-off criteria
of 1% and is therefore neglected. Packaging of the final product consist of a plastic bag and a corrugated board box.
Module C1 = The de-installation of the luminaire is done by manual labor, with the help of electrical machines. The use of portable electrical
devices (e.g., drill) usually have low energy requirements falling under the cut-off-criterion of 1% and is therefore neglected.
Module C2 = Transportation from building site to the waste treatment facility with an average distance of 300km.
Modules C3 and C4 = Waste treatment of the product follows the default values provided in EN 50693, Product Category Rules for life cycle
assessments of electronic and electrical products and systems, table G.4. This table specified how different types of raw materials used in A1 will
likely be treated during the end-of-life of the product. Waste treatments in C3 include material recycling and incineration with and without energy
recovery and fly ash extraction. Disposal in C4 consist of landfilling of different waste fractions and of ashes.
Module D = The recyclability of metals, plastics, and electronic components allows the producers a credit for the net scrap that is produced at the
end of a product’s life. The benefits from recycling of net scrap are described in formula from EN 15804:2012+A2:2019. Substitution of heat and
electricity generated by the incineration with energy recovery of plastic insulation and other parts is also calculated in module D.
Capacity utilisation Value
Transport from production place to user (A4) Distance (km) Fuel/Energy Consumption Unit
(incl. return) % (Liter/tonne)
Truck, 16-32 tonnes, EURO 6 (km) 36,7 % 900 0,043 l/tkm 38,70
Assembly (A5) Unit Value
Waste, cardboard and paper, to average treatment
kg 0,20
- A5 including transport (kg)
Waste, plastic, mixture, to average treatment - A5
kg 0,07
including transport (kg)
Capacity utilisation Value
Transport to waste processing (C2) Distance (km) Fuel/Energy Consumption Unit
(incl. return) % (Liter/tonne)
Truck, 16-32 tonnes, EURO 6 (km) 36,7 % 300 0,043 l/tkm 12,90
Waste processing (C3) Unit Value
Aluminium to recycling (kg) kg 2,38
Copper to recycling (kg) kg 0,11
Steel to recycling (kg) kg 0,18
Waste treatment of hazardous waste, incineration
kg 0,23
with fly ash extraction (kg)
Waste treatment of non-hazardous waste,
incineration with energy recovery and fly ash kg 0,05
extraction (kg)
Waste treatment of plastic mixture, incineration
kg 1,34
with energy recovery and fly ash extraction (kg)
Waste treatment per kg electronics scrap from
LED plate, without components, recycling of kg 0,23
copper - C3 (kg)
Waste treatment per kg electronics scrap from
PWB, with components, recycling of metals C3 kg 0,06
(kg)
Waste treatment per kg used electronic cable,
kg 0,01
manual seperation (kg)
Waste treatment per kg used electronic
kg 0,51
components, manual seperation (kg)
Waste treatment per kg used electronic LED driver,
kg 0,21
manual seperation (kg)
Waste treatment per kg used electronic plug
kg 0,00
connector, manual seperation (kg)
Waste treatment per kg used PWB, shredding and
kg 0,58
separation - C3 (kg)
6 / 13
Disposal (C4) Unit Value
Landfilling of aluminium (kg) kg 1,02
Landfilling of ashes from incineration of
Hazardous waste, process per kg ashes and kg 0,04
residues - C4 (kg)
Landfilling of ashes from incineration of Non-
hazardous waste, process per kg ashes and kg 0,01
residues (kg)
Landfilling of ashes from incineration of Plastic
kg 0,05
mixture, process per kg ashes and residues (kg)
Landfilling of copper (kg) kg 0,07
Landfilling of hazardous waste (kg) kg 0,33
Landfilling of non-hazardous waste (kg) kg 0,05
Landfilling of plastic mixture (kg) kg 1,34
Landfilling of steel (kg) kg 0,05
Benefits and loads beyond the system
Unit Value
boundaries (D)
Substitution of copper with net scrap from PWB,
kg 0,02
without components (kg)
Substitution of electricity, in Norway (MJ) MJ 2,11
Substitution of primary aluminium with net scrap
kg 0,94
(kg)
Substitution of primary copper with net scrap (kg) kg 0,11
Substitution of primary metals with net scrap
kg 0,02
from PWB, with components (kg)
Substitution of primary steel with net scrap (kg) kg 0,12
Substitution of thermal energy, district heating, in
MJ 31,87
Norway (MJ)
7 / 13
LCA: Results
The LCA results are presented below for the declared unit defined on page 2 of the EPD document.
Environmental impact
Indicator Unit A1 A2 A3 A4 A5 C1 C2 C3 C4 D
GWP-total
kg CO2 -
1,54E+02 7,89E-01 3,94E+00 1,14E+00 3,49E-01 0,00E+00 3,79E-01 3,91E+00 3,01E-01 -1,02E+01
eq
GWP-fossil
kg CO2 -
1,53E+02 7,88E-01 3,74E+00 1,14E+00 9,10E-03 0,00E+00 3,79E-01 3,83E+00 2,61E-01 -9,97E+00
eq
GWP-biogenic
kg CO2 -
1,37E-01 2,47E-04 1,94E-01 4,71E-04 3,40E-01 0,00E+00 1,57E-04 8,50E-02 4,00E-02 -4,31E-02
eq
GWP-luluc
kg CO2 -
2,92E-01 4,73E-04 1,13E-02 4,05E-04 1,52E-06 0,00E+00 1,35E-04 6,19E-04 6,26E-04 -1,66E-01
eq
kg
ODP CFC11 - 9,07E-06 1,70E-07 2,03E-07 2,58E-07 1,04E-09 0,00E+00 8,59E-08 7,23E-08 1,34E-08 -1,35E-02
eq
mol H+
AP 1,10E+00 1,92E-02 1,40E-02 3,27E-03 2,26E-05 0,00E+00 1,09E-03 2,06E-03 6,01E-04 -1,77E-01
-eq
EP-FreshWater kg P -eq 1,88E-02 4,09E-06 2,58E-04 9,08E-06 3,86E-08 0,00E+00 3,03E-06 1,84E-05 3,98E-06 -1,08E-03
EP-Marine kg N -eq 1,56E-01 4,70E-03 2,76E-03 6,47E-04 1,17E-05 0,00E+00 2,16E-04 5,98E-04 3,84E-04 -1,32E-02
mol N -
EP-Terrestial 1,76E+00 5,23E-02 3,63E-02 7,23E-03 8,08E-05 0,00E+00 2,41E-03 6,40E-03 1,76E-03 -1,65E-01
eq
kg
POCP NMVOC 5,35E-01 1,37E-02 8,36E-03 2,77E-03 2,43E-05 0,00E+00 9,24E-04 1,65E-03 6,89E-04 -5,07E-02
-eq
ADP- kg Sb -
1,71E-02 1,02E-05 2,86E-05 3,14E-05 1,10E-07 0,00E+00 1,05E-05 2,92E-06 6,65E-07 -1,78E-03
minerals&metals1 eq
ADP-fossil1 MJ 1,87E+03 1,06E+01 4,93E+01 1,72E+01 6,95E-02 0,00E+00 5,73E+00 4,10E+00 1,55E+00 -1,26E+02
WDP1 m3 6,34E+03 4,61E+00 5,91E+02 1,66E+01 1,43E-01 0,00E+00 5,54E+00 2,17E+01 1,56E+01 -4,80E+03
GWP total Global Warming Potential total; GWP fossil Global Warming Potential fossil fuels ; GWP biogenic Global Warming Potential biogenic; GWP luluc Global W
Potential land use change; ODP Ozone Depletion; AP Acidification; EP freshwater Eutrophication aquatic freshwater; EP marine Eutrophication aquatic marine; EP
terrestrial Eutrophication terrestrial ;POCP Photochemical zone formation; ADPE Abiotic Depletion Potential minerals and metals; ADPf Abiotic Depletion Potential fossil
fuels;
"Reading example: 9,0 E-03 = 9,0*10-3 = 0,009"
*INA Indicator Not Assessed
1. The results of this environmental impact indicator shall be used with care as the uncertainties on these results are high or as there is limited experienced with the
indicator
Remarks to environmental impacts
The product is compliant with the European RoHS Directive 2011/65/EU on Restriction of the use of certain Hazardous Substances in Electrical and
Electronic equipment and with the European REACH regulation (EC) No 1907/2006 on Registration, Evaluation, Authorization and Restriction of
Chemicals.
8 / 13
Additional environmental impact indicators
Indicator Unit A1 A2 A3 A4 A5 C1 C2 C3 C4 D
PM Disease incidence 9,07E-06 1,32E-08 1,69E-07 6,96E-08 3,56E-10 0,00E+00 2,32E-08 1,88E-08 1,06E-08 -9,20E-07
IRP2 kgBq U235 -eq 5,85E+00 4,56E-02 2,08E-01 7,51E-02 3,03E-04 0,00E+00 2,50E-02 1,84E-02 5,74E-03 -5,30E-01
ETP-fw1 CTUe 7,60E+03 6,67E+00 8,44E+01 1,27E+01 8,35E-02 0,00E+00 4,25E+00 1,96E+01 7,07E+02 -1,11E+03
HTP-c1 CTUh 1,68E-07 0,00E+00 1,68E-09 0,00E+00 3,00E-12 0,00E+00 0,00E+00 1,97E-09 3,64E-10 -3,13E-08
HTP-nc1 CTUh 6,14E-06 2,64E-09 6,09E-08 1,39E-08 9,80E-11 0,00E+00 4,64E-09 8,82E-08 3,51E-09 -1,01E-06
SQP1 dimensionless 3,71E+02 3,26E+00 8,32E+01 1,20E+01 7,26E-02 0,00E+00 4,01E+00 1,19E+00 4,06E+00 -3,48E+01
PM Particulate Matter emissions; IRP Ionizing radiation – human health; ETP-fw Eco toxicity – freshwater; HTP-c Human toxicity – cancer effects; HTP-nc Human
toxicity – non cancer effects; SQP Soil Quality (dimensionless)
"Reading example: 9,0 E-03 = 9,0*10-3 = 0,009"
*INA Indicator Not Assessed
1. The results of this environmental impact indicator shall be used with care as the uncertainties on these results are high or as there is limited experienced with the
indicator
2. This impact category deals mainly with the eventual impact of low dose ionizing radiation on human health of the nuclear fuel cycle. It does not consider effects due
to possible nuclear accidents, occupational exposure nor due to radioactive waste disposal in underground facilities. Potential ionizing radiation from the soil, from
radon and from some construction materials is also not measured by this indicator.
9 / 13
Resource use
Indicator Unit A1 A2 A3 A4 A5 C1 C2 C3 C4 D
PERE MJ 1,66E+02 9,60E-02 4,86E+01 2,46E-01 1,36E-03 0,00E+00 8,20E-02 6,65E-01 3,48E-01 -5,71E+01
PERM MJ 1,64E+00 0,00E+00 0,00E+00 0,00E+00 -1,64E+00 0,00E+00 0,00E+00 0,00E+00 0,00E+00 0,00E+00
PERT MJ 1,68E+02 9,60E-02 4,86E+01 2,46E-01 -1,64E+00 0,00E+00 8,20E-02 6,65E-01 3,48E-01 -5,71E+01
PENRE MJ 1,82E+03 1,06E+01 4,94E+01 1,72E+01 6,95E-02 0,00E+00 5,73E+00 4,10E+00 1,55E+00 -1,26E+02
PENRM MJ 8,07E+01 0,00E+00 0,00E+00 0,00E+00 -3,15E+00 0,00E+00 0,00E+00 -7,82E+01 0,00E+00 0,00E+00
PENRT MJ 1,87E+03 1,06E+01 6,26E+01 1,72E+01 -3,08E+00 0,00E+00 5,73E+00 -7,41E+01 1,55E+00 -1,37E+02
SM kg 2,31E+00 0,00E+00 2,02E-03 0,00E+00 5,74E-05 0,00E+00 0,00E+00 1,19E-03 1,33E-02 1,23E+00
RSF MJ 1,04E+00 2,88E-03 1,22E+00 8,81E-03 4,07E-05 0,00E+00 2,94E-03 1,29E-02 2,19E-03 -6,53E-03
NRSF MJ -1,49E+00 2,27E-02 1,12E+00 3,15E-02 1,44E-04 0,00E+00 1,05E-02 -4,85E-03 6,30E-02 -7,58E-01
FW m3 1,33E+00 7,29E-04 1,32E-01 1,84E-03 3,42E-05 0,00E+00 6,13E-04 7,01E-03 1,47E-03 -2,47E-01
PERE Use of renewable primary energy excluding renewable primary energy resources used as raw materials; PERM Use of renewable primary energy resources used as
raw materials; PERT Total use of renewable primary energy resources; PENRE Use of non renewable primary energy excluding non-renewable primary energy resources
used as raw materials; PENRM Use of non renewable primary energy resources used as raw materials; PENRT Total use of non renewable primary energy resources; SM
Use of secondary materials; RSF Use of renewable secondary fuels; NRSF Use of non renewable secondary fuels; FW Use of net fresh water
"Reading example: 9,0 E-03 = 9,0*10-3 = 0,009"
*INA Indicator Not Assessed
10 / 13
End of life - Waste
Indicator Unit A1 A2 A3 A4 A5 C1 C2 C3 C4 D
HWD kg 7,90E-01 4,80E-04 3,50E-02 8,87E-04 2,09E-04 0,00E+00 2,96E-04 1,09E-03 3,73E-01 2,69E-02
NHWD kg 1,99E+01 1,76E-01 3,57E-01 8,36E-01 3,90E-02 0,00E+00 2,79E-01 1,23E-01 2,61E+00 -2,86E+00
RWD kg 4,67E-03 7,31E-05 1,44E-04 1,17E-04 4,62E-07 0,00E+00 3,90E-05 1,93E-05 6,60E-06 -4,92E-04
HWD Hazardous waste disposed; NHWD Non-hazardous waste disposed; RWD Radioactive waste disposed;
"Reading example: 9,0 E-03 = 9,0*10-3 = 0,009"
*INA Indicator Not Assessed
End of life - Output flow
Indicator Unit A1 A2 A3 A4 A5 C1 C2 C3 C4 D
CRU kg 0,00E+00 0,00E+00 0,00E+00 0,00E+00 0,00E+00 0,00E+00 0,00E+00 0,00E+00 0,00E+00 0,00E+00
MFR kg 5,55E-02 0,00E+00 3,37E+00 0,00E+00 2,24E-01 0,00E+00 0,00E+00 2,67E+00 7,11E-03 1,05E+00
MER kg 1,48E-03 0,00E+00 1,40E-05 0,00E+00 4,41E-07 0,00E+00 0,00E+00 1,39E-04 1,57E-04 -5,65E-04
EEE MJ 1,30E-02 0,00E+00 1,15E-01 0,00E+00 1,19E-02 0,00E+00 0,00E+00 2,11E+00 1,57E-03 5,93E-02
EET MJ 1,96E-01 0,00E+00 1,75E+00 0,00E+00 1,80E-01 0,00E+00 0,00E+00 3,19E+01 2,38E-02 8,97E-01
CRU Components for re-use; MFR Materials for recycling; MER Materials for energy recovery; EEE Exported electrical energy; EET Exported Energy Thermal
"Reading example: 9,0 E-03 = 9,0*10-3 = 0,009"
*INA Indicator Not Assessed
Biogenic Carbon Content
Indicator Unit At the factory gate
Biogenic carbon content in product kg C 0,00E+00
Biogenic carbon content in accompanying packaging kg C 9,26E-02
Note: 1 kg biogenic carbon is equivalent to 44/12 kg CO2
11 / 13
Additional Norwegian requirements
Greenhouse gas emissions from the use of electricity in the manufacturing phase
National production mix from import, low voltage (production of transmission lines, in addition to direct emissions and losses in grid) of applied
electricity for the manufacturing process (A3).
Electricity mix Data source Amount Unit
Electricity, Denmark (kWh) ecoinvent 3.6 338,20 g CO2-eq/kWh
Dangerous substances
The product contains substances given by the REACH Candidate list and the Norwegian priority list that are less than 0,1 % by weight.
Name CASNo Amount
Lead 7439-92-1 <0,1%
Indoor environment
No effect on indoor environment.
Additional Environmental Information
Environmental impact indicators EN 15804+A1 and NPCR Part A v2.0
Indicator Unit A1 A2 A3 A4 A5 C1 C2 C3 C4 D
GWP kg CO2 -eq 1,44E+02 7,82E-01 4,91E+00 1,13E+00 3,48E-01 0,00E+00 3,75E-01 3,89E+00 2,52E-01 -8,78E+00
ODP kg CFC11 -eq 8,95E-06 1,61E-07 2,05E-07 2,09E-07 8,33E-10 0,00E+00 6,96E-08 6,78E-08 1,20E-08 -6,99E-07
POCP kg C2H4 -eq 5,09E-02 4,14E-04 7,01E-04 1,37E-04 1,20E-06 0,00E+00 4,58E-05 6,53E-05 8,09E-05 -5,86E-03
AP kg SO2 -eq 8,32E-01 1,53E-02 1,06E-02 2,25E-03 1,13E-05 0,00E+00 7,49E-04 1,57E-03 3,70E-04 -8,41E-02
EP kg PO43- -eq 1,09E-01 1,64E-03 2,09E-03 2,39E-04 3,75E-06 0,00E+00 7,97E-05 3,25E-04 1,53E-04 -5,34E-03
ADPM kg Sb -eq 1,65E-02 1,02E-05 2,86E-05 3,14E-05 1,10E-07 0,00E+00 1,05E-05 2,93E-06 6,84E-07 -2,35E-04
ADPE MJ 1,58E+03 1,05E+01 4,88E+01 1,68E+01 6,77E-02 0,00E+00 5,61E+00 3,68E+00 1,47E+00 -9,36E+01
GWPIOBC kg CO2 -eq 1,52E+02 7,89E-01 4,76E+00 1,14E+00 0,00E+00 0,00E+00 3,79E-01 3,89E+00 4,26E-02 -9,71E+00
GWP Global warming potential; ODP Depletion potential of the stratospheric ozone layer; POCP Formation potential of tropospheric photochemical oxidants; AP
Acidification potential of land and water; EP Eutrophication potential; ADPM Abiotic depletion potential for non fossil resources; ADPE Abiotic depletion​ potential for
fossil resources; GWP-IOBC/GHG Global warming potential calculated according to the principle of instantanious oxidation (except emissions and uptake of biogenic
carbon)
12 / 13
Bibliography
ISO 14025:2010. Environmental labels and declarations - Type III environmental declarations - Principles and procedures. International
Organization for Standardization.
ISO 14044:2006. Environmental management - Life cycle assessment - Requirements and guidelines. International Organization for
Standardization.
EN 15804:2012+A2:2019. Environmental product declaration - Core rules for the product category of construction products. European
Committee for Standardization.
ISO 21930:2017. Sustainability in buildings and civil engineering works - Core rules for environmental product declarations of construction
products. International Organization for Standardization.
EN 50693:2019. Product category rules for life cycle assessments of electronic and electrical products and systems. European Committee for
Standardization.
Ecoinvent v3, 2019. Allocation, cut-off by classification. Swiss Centre of Life Cycle Inventories.
Iversen et al., (2021). eEPD v2021.09, background information for EPD generator tool system verification, LCA.no. Report number: 07.21. System
verification report.
Philis et al., (2022). EPD generator for IBU PCR part B for luminaires, lamps, and components for luminaires, background information for EPD
generator application and LCA data, LCA.no. Report number: 04.22. PCR verification report.
EPD Norway (2022). NPCR Part A: Construction products and services. The Norwegian EPD foundation. Version 2.0 published 24.03.2021.
IBU (2017). PCR part B for luminaires, lampes and components for luminaires. Institut Bauen und Umwelt e.V. Version 1.7, published 30.11.2017.
Program operator and publisher Phone: +47 23 08 80 00
The Norwegian EPD Foundation e-mail: post@epd-norge.no
Post Box 5250 Majorstuen, 0303 Oslo, Norway web: www.epd-norge.no
Owner of the declaration: Phone: +47 97 66 22 12
Elektroskandia Norge AS e-mail: pkr@elektroskandia.no
Postboks 143, 1403 Langhus web: elektroskandia.no
Author of the Life Cycle Assessment Phone: +47 916 50 916
LCA.no AS e-mail: post@lca.no
Dokka 6B, 1671 web: www.lca.no
Developer of EPD generator Phone: +47 916 50 916
LCA.no AS e-mail: post@lca.no
Dokka 6B,1671 Kråkerøy web: www.lca.no
ECO Platform web: www.eco-platform.org
ECO Portal web: ECO Portal
13 / 13
