Environmental product declaration
in accordance with ISO 14025 and EN 15804+A2
Dalapro Lightning Medium Plus
Owner of the declaration: Program operator:
Saint-Gobain Sweden AB, Scanspac The Norwegian EPD Foundation
Product: Declaration number:
Dalapro Lightning Medium Plus
NEPD-8743-8395
Declared unit:
1 kg Registration number:
This declaration is based on Product Category Rules: NEPD-8743-8395
CEN Standard EN 15804:2012+A2:2019 serves as core
Issue date: 15.01.2025
PCR
The Norwegian EPD Foundation NPCR 009:2021 Part B for Technical - Chemical products Valid to: 15.01.2030
for building and construction industry
EPD software:
LCAno EPD generator ID: 739601
1 / 11
General information
Product Owner of the declaration:
Dalapro Lightning Medium Plus Saint-Gobain Sweden AB, Scanspac
Contact person: Christian Borgenfalk
Phone: +46 (0)19-46 34 00
e-mail: ehs.scanspac@dalapro.com
Program operator: Manufacturer:
The Norwegian EPD Foundation Saint-Gobain Sweden AB, Scanspac
Post Box 5250 Majorstuen, 0303 Oslo, Norway
Phone: +47 977 22 020
web: www.epd-norge.no
Declaration number: Place of production:
Saint-Gobain Sweden AB, Scanspac
NEPD-8743-8395
Kemivägen 7
SE-705 97 Glanshammar, Sweden
This declaration is based on Product Category Rules: Management system:
CEN Standard EN 15804:2012+A2:2019 serves as core PCR ISO 9001, ISO 14001
NPCR 009:2021 Part B for Technical - Chemical products for building
and construction industry
Statement of liability: Organisation no:
The owner of the declaration shall be liable for the underlying 556241-2592
information and evidence. EPD Norway shall not be liable with respect
to manufacturer information, life cycle assessment data and
evidences.​
Declared unit: Issue date:
1 kg Dalapro Lightning Medium Plus
15.01.2025
Declared unit with option: Valid to:
A1,A2,A3,A4,C1,C2,C3,C4,D 15.01.2030
Year of study:
2022
Functional unit: Comparability:
EPD of construction products may not be comparable if they not
comply with EN 15804 and seen in a building context.
General information on verification of EPD from EPD tools: Development and verification of EPD:
Independent verification of data, other environmental information The declaration is created using EPD tool lca.tools ver EPD2022.03,
and the declaration according to ISO 14025:2010, § 8.1.3 and § 8.1.4. developed by LCA.no. The EPD tool is integrated in the company's
Verification of each EPD is made according to EPD-Norway’s management system, and has been approved by EPD Norway.
guidelines for verification and approval requiring that tools are i)
integrated into the company's environmental management system, ii) Developer of EPD: Ellinor Johansson
the procedures for use of the EPD tool are approved by EPD-Norway,
Reviewer of company-specific input data and EPD: Christian
and iii) the process is reviewed annually by an independent third
Borgenfalk
party verifier. See Appendix G of EPD-Norway's General Programme
Instructions for further information on EPD tools
Verification of EPD tool: Approved:
Independent third party verification of the EPD tool, background data
and test-EPD in accordance with EPDNorway's procedures and
guidelines for verification and approval of EPD tools.
Third party verifier:
Anne Rønning, Norsus AS
(no signature required)
2 / 11
Product
Product description:
Dalapro Lightning Medium Plus is a ready-mixed all-round filler. This spray filler has good filling capacity and the smooth consistency makes it
easy to work with. Suitable for initial filling, joint filling and thin smoothing. Suitable for most substrates in new construction and renovation. Grey.
Nordic Ecolabelled.
Product specification
Packaging:
Dalapro Lightning Medium Plus 15L plastic bag
Materials Value Unit
Filler Dolomite 50-75 %
Water 20-50 %
Filler Perlite 2,5-10 %
Binder 2,5-10 %
Thickener 1-2,5 %
Additives 1-2,5 %
Packaging
Pallet
Technical data:
Binding agent: Latex co-polymer
Solvent: Water
Grain size: Max. 0,20 mm
pH: Approx. 9
Colour: Grey
Market:
Europe
Reference service life, product
Filler has a limited shelf life and is date-marked. Unopened packaging can be kept in a dark place, free from frost, for up to 12 months. Containers
that have been opened must be sealed well.
Reference service life, building
LCA: Calculation rules
Declared unit:
1 kg Dalapro Lightning Medium Plus
Cut-off criteria:
All major raw materials and all the essential energy is included. The production processes for raw materials and energy flows with very small
amounts (less than 1%) are not included. These cut-off criteria do not​ apply for hazardous materials and substances.
Allocation:
The allocation is made in accordance with the provisions of EN 15804. Incoming energy and water and waste production in-house is allocated
equally among all products through mass allocation. Effects of primary production of recycled materials is allocated to the main product in which
the material was used. The recycling process and transportation of the material is allocated to this analysis.
Data quality:
Specific data for the product composition are provided by the manufacturer. The data represent the production of the declared product and were
collected for EPD development in the year of study. Background data is based on EPDs according to EN 15804 and different LCA databases. The
data quality of the raw materials in A1 is presented in the table below.
Materials Source Data quality Year
Additives ecoinvent 3.6 Database 2019
Binder Modified ecoinvent 3.6 Database 2019
Cellulose Ether ecoinvent 3.6 Database 2019
Chemical LCA.no Database 2024
Filler ecoinvent 3.6 Database 2019
Packaging ecoinvent 3.6 Database 2019
Packaging Modified ecoinvent 3.6 Database 2019
Water ecoinvent 3.6 Database 2019
3 / 11
System boundaries (X=included, MND=module not declared, MNR=module not relevant)
Construction Beyond the system
Product stage Use stage End of life stage
installation stage boundaries
A1 A2 A3 A4 A5 B1 B2 B3 B4 B5 B6 B7 C1 C2 C3 C4 D
X X X X MND MND MND MND MND MND MND MND X X X X X
System boundary:
A1-A5: All processes from raw material extraction, transport of raw material to production site, production, transport to the construction site and
assembly are included in the analysis.
B1-B5: The user stage is not considered in this EPD.
C1-C4 and D: End of life stage and phases beyond the system boundary is part of the EPD.
System boundaries shows in the picture below.
Additional technical information:
The product meets CE-marking requirements in accordance with EN 13963.
waR slairetam tropsnarT gnirutcafunaM tropsnarT ylbmessA e​sU ecnanetniaM riapeR tnemecalpeR tnemhsibrufeR lanoitarepO ygrene esu lanoitarepO esu retaw -eD noitcurtsnoc noitilomed tropsnarT etsaW gnissecorp lasopsiD -yrevoceR-esueR laitnetop-gnilcyceR
4 / 11
LCA: Scenarios and additional technical information
The following information describe the scenarios in the different modules of the EPD.
Capacity utilisation Value
Transport from production place to user (A4) Distance (km) Fuel/Energy Consumption Unit
(incl. return) % (Liter/tonne)
Truck, over 32 tonnes, EURO 6 53,3 % 300 0,023 l/tkm 6,90
Waste processing (C3) Unit Value
Waste treatment of product after demolition (kg) kg 0,90
Disposal (C4) Unit Value
Disposal of product in landfill (kg) kg 0,10
Benefits and loads beyond the system
Unit Value
boundaries (D)
Substitution of primary aggregates with crushed
kg 0,90
recycled products (kg)
5 / 11
LCA: Results
The LCA results are presented below for the declared unit defined on page 2 of the EPD document.
Environmental impact
Indicator Unit A1 A2 A3 A4 C1 C2 C3 C4 D
GWP-total kg CO2 -eq 2,36E-02 9,63E-03 1,32E-02 2,61E-02 0 0 6,48E-04 8,22E-04 -2,10E-03
GWP-fossil kg CO2 -eq 8,50E-02 9,63E-03 1,18E-02 2,61E-02 0 0 6,39E-04 8,20E-04 -2,06E-03
GWP-biogenic kg CO2 -eq -6,15E-02 3,54E-06 1,45E-03 1,12E-05 0 0 5,52E-06 9,58E-07 -4,11E-05
GWP-luluc kg CO2 -eq 9,03E-05 4,25E-06 6,74E-06 7,96E-06 0 0 8,84E-07 2,02E-07 -1,39E-06
ODP kg CFC11 -eq 7,56E-09 2,19E-09 6,23E-10 6,30E-09 0 0 1,25E-10 3,10E-10 -3,75E-10
AP mol H+ -eq 4,75E-04 1,36E-04 8,42E-05 8,41E-05 0 0 5,17E-06 7,30E-06 -1,85E-05
EP-FreshWater kg P -eq 5,23E-06 6,24E-08 4,27E-07 2,08E-07 0 0 4,04E-08 9,30E-09 -5,48E-08
EP-Marine kg N -eq 8,31E-05 3,37E-05 5,81E-05 1,84E-05 0 0 1,52E-06 2,71E-06 -6,43E-06
EP-Terrestial mol N -eq 9,72E-04 3,74E-04 3,82E-04 2,05E-04 0 0 1,75E-05 2,99E-05 -7,56E-05
POCP kg NMVOC -eq 3,33E-04 1,03E-04 6,65E-05 8,07E-05 0 0 4,68E-06 8,57E-06 -2,00E-05
ADP-minerals&metals1 kg Sb-eq 1,20E-06 1,33E-07 8,14E-08 4,66E-07 0 0 8,11E-09 7,39E-09 -1,83E-07
ADP-fossil1 MJ 2,02E+00 1,43E-01 4,36E-02 4,24E-01 0 0 1,98E-02 2,26E-02 -3,49E-02
WDP1 m3 5,94E+00 8,39E-02 -9,31E-01 3,25E-01 0 0 2,19E+00 1,39E-01 -1,63E+00
GWP-total = Global Warming Potential total; GWP-fossil = Global Warming Potential fossil fuels; GWP-biogenic = Global Warming Potential biogenic; GWP-luluc =
Global Warming Potential land use and land use change; ODP = Depletion potential of the stratospheric ozone layer; AP = Acidification potential, Accumulated
Exceedance; EP-freshwater = Eutrophication potential, fraction of nutrients reaching freshwater end compartment: EP-marine = Eutrophication potential, fraction of
nutrients reaching marine end compartment; EP-terrestrial = Eutrophication potential, Accumulated Exceedance; POCP = Formation potential of tropospheric ozone;
ADP-minerals&metals = Abiotic depletion potential for non-fossil resources; ADP-fossil = Abiotic depletion for fossil resources potential; WDP = Water (user)
deprivation potential, deprivation-weighted water consumption
"Reading example: 9,0 E-03 = 9,0*10-3 = 0,009"
*INA Indicator Not Assessed
1. The results of this environmental impact indicator shall be used with care as the uncertainties on these results are high or as there is limited experienced with the
indicator
Remarks to environmental impacts
6 / 11
Additional environmental impact indicators
Indicator Unit A1 A2 A3 A4 C1 C2 C3 C4 D
PM Disease incidence 3,85E-09 5,59E-10 1,42E-09 2,40E-09 0 0 8,20E-11 1,56E-10 -3,96E-10
IRP2 kgBq U235 -eq 4,81E-03 6,20E-04 1,55E-04 1,85E-03 0 0 3,33E-04 1,03E-04 -3,20E-04
ETP-fw1 CTUe 2,88E+00 9,75E-02 1,34E-01 3,10E-01 0 0 1,41E-02 1,23E-02 -3,59E-02
HTP-c1 CTUh 4,10E-11 0,00E+00 1,00E-11 0,00E+00 0 0 0,00E+00 0,00E+00 -2,00E-12
HTP-nc1 CTUh 1,09E-09 7,20E-11 3,08E-10 3,00E-10 0 0 1,20E-11 7,00E-12 -4,30E-11
SQP1 dimensionless 2,67E+00 1,18E-01 1,47E+00 4,87E-01 0 0 1,12E-02 8,69E-02 7,91E-02
PM = Particulate Matter emissions; IRP = Ionizing radiation – human health; ETP-fw = Eco toxicity – freshwater; HTP-c = Human toxicity – cancer effects; HTP-nc =
Human toxicity – non cancer effects; SQP = Potential Soil Quality Index (dimensionless)
"Reading example: 9,0 E-03 = 9,0*10-3 = 0,009"
*INA Indicator Not Assessed
1. The results of this environmental impact indicator shall be used with care as the uncertainties on these results are high or as there is limited experienced with the
indicator
2. This impact category deals mainly with the eventual impact of low dose ionizing radiation on human health of the nuclear fuel cycle. It does not consider effects due
to possible nuclear accidents, occupational exposure nor due to radioactive waste disposal in underground facilities. Potential ionizing radiation from the soil, from
radon and from some construction materials is also not measured by this indicator.
7 / 11
Resource use
Indicator Unit A1 A2 A3 A4 C1 C2 C3 C4 D
PERE MJ 2,70E-01 1,53E-03 1,34E-01 5,34E-03 0 0 1,02E-02 8,08E-04 -8,16E-03
PERM MJ 6,67E-01 0,00E+00 0,00E+00 0,00E+00 0 0 0,00E+00 0,00E+00 0,00E+00
PERT MJ 9,37E-01 1,53E-03 1,34E-01 5,34E-03 0 0 1,02E-02 8,08E-04 -8,16E-03
PENRE MJ 1,81E+00 1,43E-01 4,36E-02 4,24E-01 0 0 1,99E-02 2,26E-02 -3,68E-02
PENRM MJ 1,50E+00 0,00E+00 0,00E+00 0,00E+00 0 0 0,00E+00 0,00E+00 0,00E+00
PENRT MJ 2,08E+00 1,43E-01 4,36E-02 4,24E-01 0 0 1,99E-02 2,26E-02 -3,68E-02
SM kg 0,00E+00 0,00E+00 4,90E-04 0,00E+00 0 0 0,00E+00 0,00E+00 0,00E+00
RSF MJ 6,40E-03 5,04E-05 9,46E-05 1,87E-04 0 0 0,00E+00 1,68E-05 -1,67E-04
NRSF MJ 1,34E-03 2,41E-04 6,00E-04 6,26E-04 0 0 0,00E+00 3,62E-05 -1,72E-04
FW m3 2,12E-03 1,35E-05 4,82E-04 4,83E-05 0 0 3,40E-05 2,78E-05 -1,28E-03
PERE = Use of renewable primary energy excluding renewable primary energy resources used as raw materials; PERM = Use of renewable primary energy resources used
as raw materials; PERT = Total use of renewable primary energy resources; PENRE = Use of non renewable primary energy excluding non-renewable primary energy
resources used as raw materials; PENRM = Use of non renewable primary energy resources used as raw materials; PENRT = Total use of non renewable primary energy
resources; SM = Use of secondary materials; RSF = Use of renewable secondary fuels; NRSF = Use of non-renewable secondary fuels; FW = Net use of fresh water
"Reading example: 9,0 E-03 = 9,0*10-3 = 0,009"
*INA Indicator Not Assessed
8 / 11
End of life - Waste
Indicator Unit A1 A2 A3 A4 C1 C2 C3 C4 D
HWD kg 3,26E-04 7,25E-06 4,93E-03 2,32E-05 0 0 1,98E-06 0,00E+00 -8,40E-06
NHWD kg 8,47E-03 8,61E-03 3,73E-03 3,69E-02 0 0 6,26E-05 1,00E-01 -2,55E-04
RWD kg 4,63E-06 9,79E-07 1,86E-07 2,90E-06 0 0 2,10E-07 0,00E+00 -2,77E-07
HWD = Hazardous waste disposed; NHWD = Non-hazardous waste disposed; RWD = Radioactive waste disposed
"Reading example: 9,0 E-03 = 9,0*10-3 = 0,009"
*INA Indicator Not Assessed
End of life - Output flow
Indicator Unit A1 A2 A3 A4 C1 C2 C3 C4 D
CRU kg 0,00E+00 0,00E+00 0,00E+00 0,00E+00 0 0 0,00E+00 0,00E+00 0,00E+00
MFR kg 0,00E+00 0,00E+00 7,91E-04 0,00E+00 0 0 9,00E-01 0,00E+00 0,00E+00
MER kg 0,00E+00 0,00E+00 1,35E-02 0,00E+00 0 0 0,00E+00 0,00E+00 0,00E+00
EEE MJ 0,00E+00 0,00E+00 7,46E-03 0,00E+00 0 0 0,00E+00 0,00E+00 0,00E+00
EET MJ 0,00E+00 0,00E+00 1,13E-01 0,00E+00 0 0 0,00E+00 0,00E+00 0,00E+00
CRU = Components for re-use; MFR = Materials for recycling; MER = Materials for energy recovery; EEE = Exported energy electrical; EET = Exported energy thermal
"Reading example: 9,0 E-03 = 9,0*10-3 = 0,009"
*INA Indicator Not Assessed
Biogenic Carbon Content
Indicator Unit At the factory gate
Biogenic carbon content in product kg C 0,00E+00
Biogenic carbon content in accompanying packaging kg C 1,69E-02
Note: 1 kg biogenic carbon is equivalent to 44/12 kg CO2
9 / 11
Additional requirements
Greenhouse gas emissions from the use of electricity in the manufacturing phase
National production mix from import, low voltage (production of transmission lines, in addition to direct emissions and losses in grid) of applied
electricity for the manufacturing process (A3).
Electricity mix Source Amount Unit
Renewable electricity Saint-Gobain, based on 100% hydro power, with Guarantee of Origin from LOS 2021 (kWh) ecoinvent 3.6 4,26 g CO2-eq/kWh
Dangerous substances
The product contains no substances given by the REACH Candidate list.
Indoor environment
Additional Environmental Information
Additional environmental impact indicators required in NPCR Part A for construction products
Indicator Unit A1 A2 A3 A4 C1 C2 C3 C4 D
GWPIOBC kg CO2 -eq 8,66E-02 9,63E-03 1,26E-02 2,61E-02 0 0 6,40E-04 8,21E-04 -2,20E-03
GWP-IOBC: Global warming potential calculated according to the principle of instantaneous oxidation. In order to increase the transparency of biogenic carbon​
contribution to climate impact, the indicator GWP-IOBC is required as it declares climate impacts calculated according to the principle of instantaneous oxidation.​
GWP-IOBC is also referred to as GWP-GHG in context to Swedish public procurement legislation.
10 / 11
Bibliography
ISO 14025:2010 Environmental labels and declarations - Type III environmental declarations - Principles and procedures.
ISO 14044:2006 Environmental management - Life cycle assessment - Requirements and guidelines.
EN 15804:2012+A2:2019 Environmental product declaration - Core rules for the product category of construction products.
ISO 21930:2017 Sustainability in buildings and civil engineering works - Core rules for environmental product declarations of construction
products.
ecoinvent v3, Allocation, cut-off by classification, Swiss Centre of Life Cycle Inventories.
Iversen et al., (2021) eEPD v2021.09 Background information for EPD generator tool system verification, LCA.no Report number: 07.21
Iversen et al., (2019) EPD generator for Saint-Gobain Weber and Scanspac - Background information and LCA data, LCA.no report number 05.18
Iversen et al., (2020) EPD generator for Saint-Gobain Weber Nordics and Scanspac Background information for customer application,
and LCA data – Supplementary report for modules A5, C and D, LCA.no report number 04.20
NPCR Part A: Construction products and services. Ver. 2.0, 24.03.2021 EPD Norway.
NPCR 009 Part B for technical-chemical products. Ver. 2.0 October 2021, EPD-Norge.
Program operator and publisher Phone: +47 977 22 020
The Norwegian EPD Foundation e-mail: post@epd-norge.no
Post Box 5250 Majorstuen, 0303 Oslo, Norway web: www.epd-norge.no
Owner of the declaration: Phone: +46 (0)19-46 34 00
Saint-Gobain Sweden AB, Scanspac e-mail: ehs.scanspac@dalapro.com
Kemivägen 7 , SE-705 97 Glanshammar, Sweden web: www.dalapro.se
Author of the Life Cycle Assessment Phone: +47 916 50 916
LCA.no AS e-mail: post@lca.no
Dokka 6A, 1671 Kråkerøy, Norway web: www.lca.no
Developer of EPD generator Phone: +47 916 50 916
LCA.no AS e-mail: post@lca.no
Dokka 6A, 1671 Kråkerøy, Norway web: www.lca.no
ECO Platform web: www.eco-platform.org
ECO Portal web: ECO Portal
11 / 11
