Environmental product declaration
in accordance with ISO 14025 and EN 15804+A2
Cooker guard mKomfy Hybrid 25R
Owner of the declaration: Program operator:
CTM Lyng AS The Norwegian EPD Foundation
Product: Declaration number:
Cooker guard mKomfy Hybrid 25R
NEPD-9269-8855
Declared unit:
Registration number:
1 pcs
NEPD-9269-8855
This declaration is based on Product Category Rules:
CEN Standard EN 15804:2012+A2:2019, EN 50693:2019 Issue date: 03.03.2025
and PCR EPD Italy 007 serves as core PCR Valid to: 03.03.2030
The Norwegian EPD Foundation PCR EPD Italy 012 - Electronic and electrical products and
systems - Switches
EPD software:
LCAno EPD generator ID: 349743
1 / 14
General information
Product Owner of the declaration:
Cooker guard mKomfy Hybrid 25R CTM Lyng AS
Contact person: Vidar Gangstad
Phone: +47 40006023
e-mail: vidar@ctmlyng.no
Program operator: Manufacturer:
The Norwegian EPD Foundation CTM Lyng AS
Post Box 5250 Majorstuen, 0303 Oslo, Norway Verkstedveien 19
Phone: +47 977 22 020 7125 Vanvikan, Norway
web: www.epd-norge.no
Declaration number: Place of production:
CTM Lyng production site Vanvikan (Norway)
NEPD-9269-8855
Verkstedveien 19
7125 Vanvikan, Norway
This declaration is based on Product Category Rules: Management system:
CEN Standard EN 15804:2012+A2:2019, EN 50693:2019 and PCR NS-EN ISO 9001:2015
EPD Italy 007 serves as core PCR
PCR EPD Italy 012 - Electronic and electrical products and systems -
Switches
Statement of liability: Organisation no:
The owner of the declaration shall be liable for the underlying 936285244
information and evidence. EPD Norway shall not be liable with respect
to manufacturer information, life cycle assessment data and
evidences.​
Declared unit: Issue date:
1 pcs Cooker guard mKomfy Hybrid 25R 03.03.2025
Declared unit with option: Valid to:
A1,A2,A3,A4,A5,B6,C1,C2,C3,C4,D 03.03.2030
Year of study:
2023
Functional unit: Comparability:
1 pc of cooker guard, installed and used to protect a kitchen stove EPD of construction products may not be comparable if they not
against fire hazards, during a service life of 12 years, including waste comply with EN 15804 and seen in a building context.
treatment at end-of-life.
General information on verification of EPD from EPD tools: Development and verification of EPD:
Independent verification of data, other environmental information The declaration is created using EPD tool lca.tools ver EPD2022.03,
and the declaration according to ISO 14025:2010, § 8.1.3 and § 8.1.4. developed by LCA.no. The EPD tool is integrated in the company's
Verification of each EPD is made according to EPD-Norway’s management system, and has been approved by EPD Norway.
guidelines for verification and approval requiring that tools are i)
integrated into the company's environmental management system, ii) Developer of EPD: Vidar Gangstad - CTM Lyng AS
the procedures for use of the EPD tool are approved by EPD-Norway,
Reviewer of company-specific input data and EPD:​ Ståle Sund - CTM
and iii) the process is reviewed annually by an independent third
Lyng AS
party verifier. See Appendix G of EPD-Norway's General Programme
Instructions for further information on EPD tools
Verification of EPD tool: Approved:
2 / 14
Independent third party verification of the EPD tool, background data
and test-EPD in accordance with EPDNorway's procedures and
guidelines for verification and approval of EPD tools. Approval
number: NEPDT57.
Third party verifier:
Elisabet Amat, GREENIZE projects
(no signature required)
3 / 14
Product
Product description:
Cooker Guard with wireless sensor for ceiling or hood/extractor
Product specification
mKomfy Hybrid is a cooker guard for ceiling or hood/extractor mounting 70-210 cm over hob.
It has additional safety features and possibility of connecting additional equipment.
The sensor can be used with batteries (3xAA) or external power supply (not included).
Materials kg %
Electronic - Battery alkaline 0,07 17,00
Electronic - Cable 0,09 21,49
Electronic - Capacitor 0,00 0,74
Electronic - Diode 0,00 0,09
Electronic - Inductor 0,00 0,58
Electronic - Integrated circuit 0,00 0,42
Electronic - LED chip 0,00 0,01
Electronic - Printed wiring board 0,03 6,64
Electronic - Resistor 0,00 0,19
Electronic - Switch 0,00 0,22
Electronic - Transistor 0,00 0,01
Electronic - Unspecified 0,02 5,07
Plastic - Polyethylene (LDPE) 0,00 0,04
Plastic compound - PC and ABS 0,04 10,91
Electronic - Solder material 0,00 0,03
Metal - Copper 0,01 1,91
Metal - Stainless steel 0,00 0,71
Metal - Steel 0,00 1,11
Tape 0,00 0,30
Plastic - Acrylonitrile butadiene
0,12 28,59
styrene (ABS)
Plastic - Polycarbonate (PC) 0,02 3,96
Total 0,41 100,00
Packaging kg %
Packaging - Cardboard 0,04 51,13
Packaging - Paper 0,04 47,99
Packaging - Plastic 0,00 0,87
Total incl. packaging 0,50 100,00
Technical data:
Link to the CE Declaration and product data on our website:
https://ctmlyng.no/produkter/komfyrvakt-mkomfy-hybrid-25r/
Market:
Norway.
Reference service life, product
12 years. Estimated based on the characteristics of the product and the intended application.
Reference service life, building or construction works
60 years. Standard service life for buildings according to the PCR Part A of EPD Norway.
LCA: Calculation rules
Declared unit:
1 pcs Cooker guard mKomfy Hybrid 25R
Cut-off criteria:
All major raw materials and all the essential energy is included. The production processes for raw materials and energy flows with very small
amounts (less than 1%) are not included. These cut-off criteria do not​ apply for hazardous materials and substances.
Allocation:
The allocation is made in accordance with the provisions of EN 15804. Incoming energy and water and waste production in-house is allocated
equally among all products through mass allocation. Effects of primary production of recycled materials is allocated to the main product in which
the material was used. The recycling process and transportation of the material is allocated to this analysis.
Data quality:
4 / 14
Specific data for the product composition are provided by the manufacturer. The data represent the production of the declared product and were
collected for EPD development in the year of study. Background data is based on EPDs according to EN 15804 and different LCA databases. The
data quality of the raw materials in A1 is presented in the table below.
Materials Source Data quality Year
Scientific
Electronic - Battery alkaline Olivetti et al. (2011) + ecoinvent 3.6 literature + 2019
database
Electronic - Cable ecoinvent 3.6 Database 2019
Electronic - Capacitor ecoinvent 3.6 Database 2019
Electronic - Diode ecoinvent 3.6 Database 2019
Electronic - Inductor ecoinvent 3.6 Database 2019
Electronic - Integrated circuit ecoinvent 3.6 Database 2019
Scientific
Electronic - LED chip Scholand et al. (2012) + Ecoinvent 3.6 literature + 2017
database
Electronic - Printed wiring board Modified ecoinvent 3.6 Database 2019
Electronic - Resistor ecoinvent 3.6 Database 2019
Electronic - Solder material ecoinvent 3.6 Database 2019
Electronic - Switch ecoinvent 3.6 Database 2019
Electronic - Transistor ecoinvent 3.6 Database 2019
Electronic - Unspecified ecoinvent 3.6 Database 2019
Metal - Copper ecoinvent 3.6 Database 2019
Metal - Stainless steel ecoinvent 3.6 Database 2019
Metal - Steel ecoinvent 3.6 Database 2019
Packaging - Cardboard ecoinvent 3.6 Database 2019
Packaging - Paper ecoinvent 3.6 Database 2019
Packaging - Plastic ecoinvent 3.6 Database 2019
Plastic - Acrylonitrile butadiene styrene (ABS) ecoinvent 3.6 Database 2019
Plastic - Polycarbonate (PC) ecoinvent 3.6 Database 2019
Plastic - Polyethylene (LDPE) ecoinvent 3.6 Database 2019
Plastic compound - PC and ABS ecoinvent 3.6 Database 2019
Tape ecoinvent 3.6 Database 2019
5 / 14
System boundaries (X=included, MND=module not declared, MNR=module not relevant)
Construction Beyond the system
Product stage Use stage End of life stage
installation stage boundaries
A1 A2 A3 A4 A5 B1 B2 B3 B4 B5 B6 B7 C1 C2 C3 C4 D
X X X X X MND MND MND MND MND X MND X X X X X
System boundary:
Additional technical information:
waR slairetam tropsnarT gnirutcafunaM tropsnarT ylbmessA e​sU ecnanetniaM riapeR tnemecalpeR tnemhsibrufeR lanoitarepO ygrene esu lanoitarepO esu retaw -eD noitcurtsnoc noitilomed tropsnarT etsaW gnissecorp lasopsiD -yrevoceR-esueR laitnetop-gnilcyceR
6 / 14
LCA: Scenarios and additional technical information
The following information describe the scenarios in the different modules of the EPD.
Module A4 = In A4, an average transport distance from the production site in Vanvikan to the warehouses we deliver to was included. This
transport consist of 14 km by ferry and 516 km by truck. An average distance of 300 km by truck was also added as additional transport to
market.
Modules A5 = installation is done by manual labour. The use of portable electrical devices such as drills usually have low energy requirements
falling under the cut-off criterion of 1% and are therefore neglected (especially for small retail devices). No product scraps are generated during
installation, but the end-of-life treatment of packaging is systematically accounted for in this module.
Module B6 = The operational energy use of the switch is calculated based on the methodology provided in the PCR EPD Italy 012 Part B for
switches. To calculate the electricity use of the stove guard, the following scenario parameters have been applied:
- Power consumed (Puse) = 2.99 watt
- Reference service life (RSL) = 12 years
- Number of hours in a year = 8760 hours (according to section 4.2.3.5 of the PCR)
- Operating time coefficient (a) = 100 percent (according to section 4.2.3.5 of the PCR)
- Reference current = 100% (according to section 4.2.3.5 of the PCR – used to calculate Puse)
In our calculation, we have considered that the product draws current continuously, and therefore, we have used a reference current value of
100% in the calculation (instead of 50%). This represents the total load that the product imposes on the system during constant operation. We
include 3 pieces of AA batteries with the product, and have therefore also added the energy they deliver: Capacity 2.6 Ah × 3 pcs × Voltage 1.5 V
/ 1000 = Energy 0.0117 (kWh).
Module C1 = De-installation is done by manual labour. The use of portable electrical devices such as drills usually have low energy requirements
falling under the cut-off criterion of 1% and are therefore neglected (especially for small retail devices).
Module C2 = Transport from the installation site to the nearest waste treatment facility is based on an average distance of 300 km.
Modules C3 and C4 = Waste treatment of the product follows the default values provided in EN 50693, Product Category Rules for life cycle
assessments of electronic and electrical products and systems, table G.4. This table specified how different types of raw materials used in A1 will
likely be treated during the end-of-life of the product. Waste treatments in C3 include material recycling and incineration with energy recovery and
fly ash extraction. Disposal in C4 consist of landfilling of different waste fractions and of ashes.
Module D = The recyclability of metals, plastics, and electronic components allows the producers a credit for the net scrap that is produced at the
end of a product’s life. The benefits from recycling of net scrap are described in formula from EN 15804:2012+A2:2019. Substitution of heat and
electricity generated by the incineration with energy recovery of plastic insulation and other parts is also calculated in module D.
Capacity utilisation Value
Transport from production place to user (A4) Distance (km) Fuel/Energy Consumption Unit
(incl. return) % (Liter/tonne)
Truck, 16-32 tonnes, EURO 4 (km) - Europe 36,7 % 300 0,044 l/tkm 13,20
Assembly (A5) Unit Value
Waste, packaging, corrugated board box, to
kg 0,044
average treatment - A5 including transport (kg)
Waste, packaging, plastic film (LDPE), to average
kg 0,00076
treatment - A5 including transport (kg)
Waste, packaging, paper printed, to average
kg 0,041
treatment - A5 including transport (kg)
Operational energy (B6) Unit Value
Electricity, Norway (kWh) kWh/DU 314,31
Capacity utilisation Value
Transport to waste processing (C2) Distance (km) Fuel/Energy Consumption Unit
(incl. return) % (Liter/tonne)
Truck, 16-32 tonnes, EURO 5 (km) - Europe 36,7 % 300 0,044 l/tkm 13,20
7 / 14
Waste processing (C3) Unit Value
Waste treatment per kg used electronic plug
kg 0,081
connector, manual seperation (kg)
Waste treatment of plastic mixture, incineration
kg 0,11
with energy recovery and fly ash extraction (kg)
Steel to recycling (kg) kg 0,011
Copper to recycling (kg) kg 0,0074
Waste treatment per kg used PWB, shredding and
kg 0,057
separation - C3 (kg)
Waste treatment per kg electronics scrap from
PWB, with components, recycling of metals C3 kg 0,028
(kg)
Waste treatment per kg used electronic cable,
kg 0,0070
manual seperation (kg)
Waste treatment of polyethylene (PE),
incineration with energy recovery and fly ash kg 0,000075
extraction (kg)
Acrylonitrile butadiene styrene (ABS) to recycling kg 0,023
Disposal (C4) Unit Value
Landfilling of ashes from incineration of Plastic
kg 0,0040
mixture, process per kg ashes and residues (kg)
Landfilling of plastic mixture (kg) kg 0,11
Landfilling of steel (kg) kg 0,0028
Landfilling of copper (kg) kg 0,0049
Landfilling of hazardous waste (kg) kg 0,098
Landfilling of ashes from incineration of
Polyethylene (PE), process per kg ashes and kg 0,0000026
residues (kg)
Benefits and loads beyond the system
Unit Value
boundaries (D)
Substitution of electricity, in Norway (MJ) MJ 0,17
Substitution of thermal energy, district heating, in
MJ 2,70
Norway (MJ)
Substitution of primary steel with net scrap (kg) kg 0,0062
Substitution of primary copper with net scrap (kg) kg 0,0036
Substitution of primary metals with net scrap
kg 0,0084
from PWB, with components (kg)
Substitution of acrylonitrile butadiene styrene,
kg 0,023
ABS, granulate (kg)
8 / 14
LCA: Results
The LCA results are presented below for the declared unit defined on page 2 of the EPD document.
Environmental impact
Indicator Unit A1 A2 A3 A4 A5
GWP-total kg CO2 -eq 1,01E+01 2,54E-01 9,11E-03 2,47E-02 1,49E-01
GWP-fossil kg CO2 -eq 1,02E+01 2,54E-01 8,58E-03 2,46E-02 1,45E-03
GWP-biogenic kg CO2 -eq -1,13E-01 9,18E-05 4,98E-04 1,01E-05 1,48E-01
GWP-luluc kg CO2 -eq 1,68E-02 1,19E-04 3,06E-05 8,69E-06 4,65E-07
ODP kg CFC11 -eq 6,95E-07 5,60E-08 5,44E-10 5,67E-09 2,98E-10
AP mol H+ -eq 9,15E-02 3,37E-03 5,92E-05 1,25E-04 6,67E-06
EP-FreshWater kg P -eq 1,78E-03 1,74E-06 5,40E-07 1,95E-07 1,16E-08
EP-Marine kg N -eq 1,25E-02 8,19E-04 7,24E-06 4,27E-05 2,25E-06
EP-Terrestial mol N -eq 1,46E-01 9,11E-03 8,78E-05 4,71E-04 2,39E-05
POCP kg NMVOC -eq 4,37E-02 2,49E-03 2,37E-05 1,34E-04 6,88E-06
ADP-minerals&metals1 kg Sb-eq 4,67E-03 5,20E-06 5,56E-07 6,73E-07 3,42E-08
ADP-fossil1 MJ 1,32E+02 3,63E+00 1,04E-01 3,75E-01 1,97E-02
WDP1 m3 3,51E+02 2,27E+00 1,76E+01 3,57E-01 2,56E-02
Indicator Unit B6 C1 C2 C3 C4 D
GWP-total kg CO2 -eq 7,65E+00 0,00E+00 2,49E-02 3,04E-01 3,46E-02 -6,22E-01
GWP-fossil kg CO2 -eq 7,41E+00 0,00E+00 2,49E-02 3,04E-01 3,44E-02 -6,19E-01
GWP-biogenic kg CO2 -eq 2,05E-01 0,00E+00 1,01E-05 5,37E-05 1,96E-05 -1,91E-03
GWP-luluc kg CO2 -eq 3,06E-02 0,00E+00 8,69E-06 5,82E-05 1,86E-04 -1,25E-03
ODP kg CFC11 -eq 5,08E-07 0,00E+00 5,67E-09 2,34E-09 1,46E-09 -1,14E-03
AP mol H+ -eq 5,79E-02 0,00E+00 1,02E-04 1,65E-04 1,08E-04 -3,22E-02
EP-FreshWater kg P -eq 5,33E-04 0,00E+00 1,95E-07 8,44E-07 9,50E-07 -1,79E-04
EP-Marine kg N -eq 6,37E-03 0,00E+00 3,01E-05 4,80E-05 3,72E-05 -1,70E-03
EP-Terrestial mol N -eq 8,29E-02 0,00E+00 3,33E-04 5,12E-04 2,51E-04 -2,32E-02
POCP kg NMVOC -eq 2,23E-02 0,00E+00 1,02E-04 1,33E-04 1,18E-04 -6,72E-03
ADP-minerals&metals1 kg Sb-eq 5,53E-04 0,00E+00 6,73E-07 2,48E-07 1,31E-07 -7,28E-04
ADP-fossil1 MJ 1,01E+02 0,00E+00 3,75E-01 2,97E-01 2,60E-01 -8,73E+00
WDP1 m3 1,76E+04 0,00E+00 3,57E-01 3,02E+00 4,60E-01 -1,66E+01
GWP-total = Global Warming Potential total; GWP-fossil = Global Warming Potential fossil fuels; GWP-biogenic = Global Warming Potential biogenic; GWP-luluc =
Global Warming Potential land use and land use change; ODP = Depletion potential of the stratospheric ozone layer; AP = Acidification potential, Accumulated
Exceedance; EP-freshwater = Eutrophication potential, fraction of nutrients reaching freshwater end compartment: EP-marine = Eutrophication potential, fraction of
nutrients reaching marine end compartment; EP-terrestrial = Eutrophication potential, Accumulated Exceedance; POCP = Formation potential of tropospheric ozone;
ADP-minerals&metals = Abiotic depletion potential for non-fossil resources; ADP-fossil = Abiotic depletion for fossil resources potential; WDP = Water (user)
deprivation potential, deprivation-weighted water consumption
"Reading example: 9,0 E-03 = 9,0*10-3 = 0,009"
*INA Indicator Not Assessed
1. The results of this environmental impact indicator shall be used with care as the uncertainties on these results are high or as there is limited experienced with the
indicator
Remarks to environmental impacts
9 / 14
Additional environmental impact indicators
Indicator Unit A1 A2 A3 A4 A5
PM Disease incidence 5,62E-07 1,08E-08 4,28E-10 1,79E-09 9,80E-11
IRP2 kgBq U235 -eq 4,33E-01 1,56E-02 1,84E-03 1,64E-03 8,45E-05
ETP-fw1 CTUe 9,53E+02 2,55E+00 4,68E-01 2,76E-01 2,62E-02
HTP-c1 CTUh 1,24E-08 0,00E+00 2,20E-11 0,00E+00 0,00E+00
HTP-nc1 CTUh 5,79E-07 2,09E-09 5,32E-10 2,98E-10 3,30E-11
SQP1 dimensionless 4,76E+01 1,89E+00 5,27E-02 2,58E-01 1,35E-02
Indicator Unit B6 C1 C2 C3 C4 D
PM Disease incidence 4,15E-07 0,00E+00 1,79E-09 9,78E-10 1,98E-09 -7,53E-08
IRP2 kgBq U235 -eq 1,84E+00 0,00E+00 1,64E-03 1,44E-03 4,86E-04 -2,48E-02
ETP-fw1 CTUe 4,61E+02 0,00E+00 2,76E-01 1,06E+00 5,46E+00 -2,30E+02
HTP-c1 CTUh 2,20E-08 0,00E+00 0,00E+00 4,99E-10 9,40E-11 -1,25E-09
HTP-nc1 CTUh 5,18E-07 0,00E+00 2,98E-10 2,93E-08 6,78E-10 -8,52E-08
SQP1 dimensionless 5,10E+01 0,00E+00 2,58E-01 7,46E-02 6,92E-01 -6,23E+00
PM = Particulate Matter emissions; IRP = Ionizing radiation – human health; ETP-fw = Eco toxicity – freshwater; HTP-c = Human toxicity – cancer effects; HTP-nc =
Human toxicity – non cancer effects; SQP = Potential Soil Quality Index (dimensionless)
"Reading example: 9,0 E-03 = 9,0*10-3 = 0,009"
*INA Indicator Not Assessed
1. The results of this environmental impact indicator shall be used with care as the uncertainties on these results are high or as there is limited experienced with the
indicator
2. This impact category deals mainly with the eventual impact of low dose ionizing radiation on human health of the nuclear fuel cycle. It does not consider effects due
to possible nuclear accidents, occupational exposure nor due to radioactive waste disposal in underground facilities. Potential ionizing radiation from the soil, from
radon and from some construction materials is also not measured by this indicator.
10 / 14
Resource use
Indicator Unit A1 A2 A3 A4 A5
PERE MJ 1,28E+01 4,15E-02 1,31E+00 5,29E-03 3,27E-04
PERM MJ 9,53E-01 0,00E+00 0,00E+00 0,00E+00 -9,53E-01
PERT MJ 1,38E+01 4,15E-02 1,31E+00 5,29E-03 -9,53E-01
PENRE MJ 1,23E+02 3,63E+00 1,04E-01 3,75E-01 1,97E-02
PENRM MJ 1,01E+01 0,00E+00 0,00E+00 0,00E+00 -3,23E-02
PENRT MJ 1,32E+02 3,63E+00 1,04E-01 3,75E-01 -1,25E-02
SM kg 9,98E-02 0,00E+00 0,00E+00 0,00E+00 0,00E+00
RSF MJ 2,09E-01 1,30E-03 1,04E-03 1,89E-04 1,08E-05
NRSF MJ 5,69E-02 6,91E-03 2,57E-03 6,76E-04 4,43E-05
FW m3 1,03E-01 3,28E-04 9,96E-03 3,95E-05 9,33E-06
Indicator Unit B6 C1 C2 C3 C4 D
PERE MJ 1,31E+03 0,00E+00 5,29E-03 3,82E-02 8,27E-02 -2,01E+00
PERM MJ 0,00E+00 0,00E+00 0,00E+00 0,00E+00 0,00E+00 0,00E+00
PERT MJ 1,31E+03 0,00E+00 5,29E-03 3,82E-02 8,27E-02 -2,01E+00
PENRE MJ 1,01E+02 0,00E+00 3,75E-01 2,97E-01 2,60E-01 -8,73E+00
PENRM MJ 0,00E+00 0,00E+00 0,00E+00 -1,01E+01 0,00E+00 0,00E+00
PENRT MJ 1,01E+02 0,00E+00 3,75E-01 -9,80E+00 2,60E-01 -8,73E+00
SM kg 0,00E+00 0,00E+00 0,00E+00 0,00E+00 2,17E-03 4,53E-03
RSF MJ 1,03E+00 0,00E+00 1,89E-04 6,21E-04 2,05E-04 2,48E-04
NRSF MJ 2,56E+00 0,00E+00 6,76E-04 -2,90E-05 1,84E-02 -7,44E-02
FW m3 9,79E+00 0,00E+00 3,95E-05 4,98E-04 1,60E-04 -7,71E-03
PERE = Use of renewable primary energy excluding renewable primary energy resources used as raw materials; PERM = Use of renewable primary energy resources used
as raw materials; PERT = Total use of renewable primary energy resources; PENRE = Use of non renewable primary energy excluding non-renewable primary energy
resources used as raw materials; PENRM = Use of non renewable primary energy resources used as raw materials; PENRT = Total use of non renewable primary energy
resources; SM = Use of secondary materials; RSF = Use of renewable secondary fuels; NRSF = Use of non-renewable secondary fuels; FW = Net use of fresh water
"Reading example: 9,0 E-03 = 9,0*10-3 = 0,009"
*INA Indicator Not Assessed
11 / 14
End of life - Waste
Indicator Unit A1 A2 A3 A4 A5
HWD kg 4,23E-02 1,99E-04 4,84E-04 1,91E-05 0,00E+00
NHWD kg 1,11E+00 1,24E-01 8,59E-03 1,79E-02 8,69E-02
RWD kg 3,36E-04 2,47E-05 9,21E-07 2,55E-06 0,00E+00
Indicator Unit B6 C1 C2 C3 C4 D
HWD kg 6,50E-02 0,00E+00 1,91E-05 1,43E-05 9,88E-02 -1,95E-03
NHWD kg 7,79E+00 0,00E+00 1,79E-02 1,93E-02 1,25E-01 -9,50E-02
RWD kg 9,06E-04 0,00E+00 2,56E-06 7,11E-07 1,95E-07 -2,13E-05
HWD = Hazardous waste disposed; NHWD = Non-hazardous waste disposed; RWD = Radioactive waste disposed
"Reading example: 9,0 E-03 = 9,0*10-3 = 0,009"
*INA Indicator Not Assessed
End of life - Output flow
Indicator Unit A1 A2 A3 A4 A5
CRU kg 0,00E+00 0,00E+00 0,00E+00 0,00E+00 0,00E+00
MFR kg 0,00E+00 0,00E+00 3,66E-03 0,00E+00 8,05E-02
MER kg 0,00E+00 0,00E+00 2,36E-03 0,00E+00 6,02E-03
EEE MJ 0,00E+00 0,00E+00 1,53E-03 0,00E+00 4,93E-03
EET MJ 0,00E+00 0,00E+00 2,32E-02 0,00E+00 7,45E-02
Indicator Unit B6 C1 C2 C3 C4 D
CRU kg 0,00E+00 0,00E+00 0,00E+00 0,00E+00 0,00E+00 0,00E+00
MFR kg 0,00E+00 0,00E+00 0,00E+00 4,23E-02 1,05E-05 1,89E-03
MER kg 0,00E+00 0,00E+00 0,00E+00 1,16E-01 1,24E-06 -1,18E-05
EEE MJ 0,00E+00 0,00E+00 0,00E+00 1,79E-01 2,53E-05 -3,35E-05
EET MJ 0,00E+00 0,00E+00 0,00E+00 2,71E+00 3,83E-04 -5,07E-04
CRU = Components for re-use; MFR = Materials for recycling; MER = Materials for energy recovery; EEE = Exported energy electrical; EET = Exported energy thermal
"Reading example: 9,0 E-03 = 9,0*10-3 = 0,009"
*INA Indicator Not Assessed
Biogenic Carbon Content
Indicator Unit At the factory gate
Biogenic carbon content in product kg C 0,00E+00
Biogenic carbon content in accompanying packaging kg C 4,02E-02
Note: 1 kg biogenic carbon is equivalent to 44/12 kg CO2
12 / 14
Additional requirements
Greenhouse gas emissions from the use of electricity in the manufacturing phase
National production mix from import, low voltage (production of transmission lines, in addition to direct emissions and losses in grid) of applied
electricity for the manufacturing process (A3).
Electricity mix Source Amount Unit
Electricity, Norway (kWh) ecoinvent 3.6 24,33 g CO2-eq/kWh
Dangerous substances
The product contains no substances on the REACH Candidate list at or above 100 ppm, 0,01 % by weight.
Indoor environment
Additional Environmental Information
Additional environmental impact indicators required in NPCR Part A for construction products
Indicator Unit A1 A2 A3 A4 A5
GWPIOBC kg CO2 -eq 1,02E+01 2,54E-01 9,06E-03 2,47E-02 6,75E-04
Indicator Unit B6 C1 C2 C3 C4 D
GWPIOBC kg CO2 -eq 7,63E+00 0,00E+00 2,49E-02 3,04E-01 2,68E-02 -6,20E-01
GWP-IOBC: Global warming potential calculated according to the principle of instantaneous oxidation. In order to increase the transparency of biogenic carbon​
contribution to climate impact, the indicator GWP-IOBC is required as it declares climate impacts calculated according to the principle of instantaneous oxidation.​
GWP-IOBC is also referred to as GWP-GHG in context to Swedish public procurement legislation.
13 / 14
Bibliography
ISO 14025:2010. Environmental labels and declarations - Type III environmental declarations - Principles and procedures. International
Organization for Standardization.
ISO 14044:2006. Environmental management - Life cycle assessment - Requirements and guidelines. International Organization for
Standardization.
EN 15804:2012+A2:2019. Environmental product declaration - Core rules for the product category of construction products. European
Committee for Standardization.
ISO 21930:2017. Sustainability in buildings and civil engineering works - Core rules for environmental product declarations of construction
products. International Organization for Standardization.
EN 50693:2019. Product category rules for life cycle assessments of electronic and electrical products and systems. European Committee for
Standardization.
Ecoinvent v3, 2019. Allocation, cut-off by classification. Swiss Centre of Life Cycle Inventories.
Iversen et al., (2021). eEPD v2021.09, background information for EPD generator tool system verification, LCA.no. Report number: 07.21. System
verification report.
Ruud & Philis (2023). EPD generator for PCR EPD Italy 012 part B for switches, background information for EPD generator application and LCA
data, LCA.no. Report number: 01.23. PCR verification report.
EPD Italy (2020). PCR EPD Italy 007 Part A for electronic and electrical products and systems. EPD Italy. Version 3, issue 13-01-2023 and valid
until 19-01-2025.
EPD Italy (2020). PCR EPD Italy 012 Part B for switches. EPD Italy. Version 0, issue 16-03-2020 and valid until 15-03-2025.
Program operator and publisher Phone: +47 977 22 020
The Norwegian EPD Foundation e-mail: post@epd-norge.no
Post Box 5250 Majorstuen, 0303 Oslo, Norway web: www.epd-norge.no
Owner of the declaration: Phone: +47 40006023
CTM Lyng AS e-mail: vidar@ctmlyng.no
Verkstedveien 19, 7125 Vanvikan, Norway web: ctmlyng.no
Author of the Life Cycle Assessment Phone: +47 916 50 916
LCA.no AS e-mail: post@lca.no
Dokka 6A, 1671 Kråkerøy, Norway web: www.lca.no
Developer of EPD generator Phone: +47 916 50 916
LCA.no AS e-mail: post@lca.no
Dokka 6A, 1671 Kråkerøy, Norway web: www.lca.no
ECO Platform web: www.eco-platform.org
ECO Portal web: ECO Portal
14 / 14
