Environmental Product
Declaration
In accordance with ISO 14025 and EN 15804 +A2
Owner of the declaration:
Lyngson, Sia Product name:
Program holder and publisher:
Panel radiator type 22 size – h500
The Norwegian EPD foundation mm x L700 mm
Declaration number:
NEPD-3296-1940-EN
Registration Number:
NEPD-3296-1940-EN :
Issue date: Manufacturer
Valid to: Lyngson, Sia
03.01.2022
The Norwegian 03.01.2027
EPD Foundation
General information
Product:
Panel radiator type 22 size - h500 mm x L700 mm Owner of the declaration:
Lyngson, SIA
Program Operator: Contact person: Uldis Benhens
The Norwegian EPD Foundation Phone: +371 29 474 739
Post Box 5250 Majorstuen, 0303 Oslo, Norway e-mail: Uldis.Benhens@lyngson.lv
Tlf: +47 23 08 80 00
e-mail: post@epd-norge.no Manufacturer:
Lyngson, SIA
Declaration Number:
Akaci, Olaines novadas, Olaines pagasts, Latvia
Phone: +371 67796710
e-mail: info@lyngson.lv
NEPD-3296-1940-EN
This declaration is based on Product
Category Rules: Place of production:
CEN Standard EN 15804:2012+A2:2019 Akaci, Olaines novadas, Olaines pagasts, Latvia
and
Management system:
NPCR Part A Construction products and
ISO 9001, ISO 50001 and ISO 14001
services ver 2.
Statements:
Organisation no:
The owner of the declaration shall be liable for the
--
underlying information and evidence. EPD
Norway shall not be liable with respect to
Issue date:
manufacturer, life cycle assessment data and
evidences.
03.01.2022
Valid to:
Declared unit:
1 piece of Panel radiator type 22 size – h500 mm x
L700mm, capable to produce 1 kW of heating
03.01.2027
as defined by the manufacturer. Year of study:
2021
Verification:
Independent verification of the declaration and Comparability:
data, according to ISO14025:2010 EPDs from other programmes than EPD Norge
internal external ⊠ may not be comparable.
Sign
The EPD has been worked out by:
Bureau Veritas Latvia
Elisabet Amat
Independent verifier approved by EPD Norway
Approved (Manager of EPD Norway)
EPD for the best environmental decision 2
Product
Product description:
Panel heaters with compact module and side connection. These devices have a wide range of
applications in closed environments, both in new construction and renovations. It has a lifespan
of 50 years. The Panel radiator products are produced only in one plant.
Product specification:
The product composition is steel and paint.
Products materials KG %
Steel 19,5 98
Paint 0,414 2
TOTAL 19,914 100
Packaging materials KG %
Cardboard 0,35 56,45
PE 0,27 43,55
TOTAL 0,62 100
Technical data:
• Length – 700 mm, Width – 500 mm, Thickness – 102 mm;
• Weight 19,914 kg;
• Density 7,85 kg/dm3;
• Lifetime 50 years;
• Tensile strength 270 – 410 MPa;
• Water resistance for 100 h of humidity.
Market:
Nordic market
Reference service life, product:
50 years
LCA: Calculation rules
Declated unit:
1 piece of Panel radiator type 22 size – h500 mm x L700mm, capable to produce 1 kW of heating
as defined by the manufacturer. For the static or mixed hot water radiator, the measurement of
EPD for the best environmental decision 3
this power is defined at ΔT 50 according to the EN 442 standard and with a reference lifetime of
50 years.
Data quality:
The production data are from 2020, the database data are from 2013 – 2021 i.e. no data is older
than 10 years. Database used is mainly Ecoinvent 3.7.1. The LCA software used is SimaPro 9.2.
Allocation:
Heat, electricity and other energy use, and waste in production are calculated as a average weight
per produced tonne of all products using yearly production data and rate for 2020. For
manufacturing processes and raw materials the specific country mix of heat and electricity were
considered. For secondary data on materials’ flow information has been gathered from the
Ecoinvent 3.7.1 database. In addition, the allocation is made following the provisions of PSR-
0011-ed1.0-EN-2018 02 09. Incoming energy and water together with waste production in-house
are allocated equally among all products through mass allocation. The recycling process and
transportation of the material are allocated to this analysis.
System boundary:
LCA is made in “Cradle-to-gate with options, modules C1-C4 and module D ”. All major materials,
production energy use and waste are included for product stages A1, A2, A3, A4, C1, C2, C3, C4,
and D. All life cycle impacts are included, see flowchart below. The following information
describes the scenarios in the different modules of the EPD. It must be noted that, all major raw
materials and all the essential energy are included.
Cut-off criteria:
Marginal production process for raw materials and energy flows with a cut-off of 1% not included
in the Ecoinvent database are not considered. This cut-off rule does not apply for hazardous
materials and substances and it is consistent with EN 15804+A2.
EPD for the best environmental decision 4
LCA: Scenarios and additional technical information
The following information describe the scenarios in the different modules of the EPD.
Product stage (A1, A2, A3)
- Raw material supply (A1)
The materials needed for the production of a Panel radiator type 22 size - h500 mm x L700 mm
are: steel, lubricating oil, chemicals for washing (tetrachloroethylene), hydraulic gas, powder
paint (polyester resin), cardboard and packaging film (PE). The cooling liquid used in the process
has not been because of a quantity less than 1% in mass.
- Transport of raw materials (A2)
Steel is transported for a distance of 473 km, steel connection 2943 km, lubricating oil 30 km,
hydraulic gas 30 km, powder paint 25 km, cardboard 300 km, PE 3 km, and chemicals (Gardobond
H 7406, Gardobond A 4952, Gardobond H 7200L) 550 km.
- Manufacturing (A3)
This product stage includes welding, stamping, painting, assembling and packing of the final
product. It includes energy consumption (electricity, natural gas), the consumption of raw
materials such as water and some operations such as welding, as well as the waste and emissions
produced within manufacturing stage.
Transport from production place to assembly/user (A4)
Transportation from Lyngson SIA production sites in Latvia to customers in Sweden, Norway,
Finland and Estonia have been considered and described in tha table below. Trips start with an
initial transport of 30km from the production factory to the harbour of Riga from which they
follow a sea route of 440 km to Sweden and then split according to different scenarios where
products destined for Norway depart by road from Oslo with different distances 660 km, 1060
km and 1310 km. While for Finland the sea route is 400 km, instead for Estonia there is just road
transport.
Capacity utilisation (incl. Distance Fuel/Energy value
Type Type of vehicle
return) % KM consumption (l/t)
Sweden destination 1
Truck 75% Lorry, >32t, EURO6 200 0,0226 l/tkm 4,52
Boat 64% Ferry 440 0,0299 l/tkm 13,156
Sweden destination 2
Truck 75% Lorry, >32t, EURO6 600 0,0226 l/tkm 13,56
Boat 64% Ferry 440 0,0299 l/tkm 13,156
Sweden destination 3
Truck 10% Lorry, >32t, EURO6 850 0,0226 l/tkm 19,21
Boat 64% Ferry 440 0,0299 l/tkm 13,156
Norway destination 1
Truck 75% Lorry, >32t, EURO6 660 0,0226 l/tkm 14,916
Boat 64% Ferry 440 0,0299 l/tkm 13,156
EPD for the best environmental decision 5
Norway destination 2
Truck 75% Lorry, >32t, EURO6 1060 0,0226 l/tkm 23,956
Boat 64% Ferry 440 0,0299 l/tkm 13,156
Norway destination 3
Truck 15% Lorry, >32t, EURO6 1310 0,0226 l/tkm 29,606
Boat 64% Ferry 440 0,0299 l/tkm 13,156
Finland
Truck 25% Lorry, >32t, EURO6 100 0,0226 l/tkm 2,26
Boat 64% Ferry 400 0,0299 l/tkm 11,96
Estonia
Truck 25% Lorry, >32t, EURO6 400 0,0226 l/tkm 9,04
End of Life (C1, C3, C4)
- Demolition (C1)
It is assumed that for the decommissioning of a radiator there are no particular operations and
therefore in this step it is possible to exclude relavant impacts.
- Waste processing (C3)
It is assumed that there are no special procedures for preparing the radiator as a “waste”.
- Disposal (C4)
It is assumed the following scenario: for the cardboard (0,35 kg) the 74,2% is recycled, while the
remaining quantity for 95% goes to an energy recovery through incineration and 5% is disposed
of through landfill. PE (0,27 kg) is recycled for 37,5%, the remaining quantity follows the same
end as for cardboard. The quantities divided by the different fractions are shown in the following
table and for the recycling is included also the amount of steel from the radiator.
Type Unit Value
Hazardous waste disposed Kg 0
Collected as mixed construction waste Kg 0
Reuse Kg 0
Recycling Kg 19,861
Energy recovery Kg 0,247
To landfill Kg 0,013
Transport to waste processing (C2)
As suggested by PSR-0011-ed1.0-EN-2018 02 09 is assumed an average transport for a distance
of 100 km by truck.
Capacity utilisation (incl. Distance Fuel/Energy value
Type Type of vehicle
return) % KM consumption (l/t)
Truck 36,5 Lorry, 16-32t, EURO5 100 0,0449 l/tkm 4,49
EPD for the best environmental decision 6
Benefits and loads beyond the system boundaries (D)
It is assumed that all the quantity of steel that form a Panel radiator size 22 - h500 mm x L700
mm is recovered and recycled. In addition, is recycled also the 74,2% of carboard and the 37,5%
of PE from the packaging materials.
Material Unit Value
Steel kg 19,5
PE kg 0,101
Cardboard kg 0,2597
System boundaries (X=included, MND= module not declared, MNR=module not
relevant)
Benefits
& loads
Assembly
Product stage Use stage End of life stage beoyond
stage
system
boundary
EPD for the best environmental decision 7
slairetam
waR
tropsnarT
gnirutcafunaM
tropsnarT ylbmessA
esU
ecnanetniaM
riapeR
tnemecalpeR tnemhsibrufeR
esu
ygrene
lanoitarepO
esu
retaw
lanoitarepO
noitilomed
noitcurtsnoc-eD
tropsnarT
gnissecorp
etsaW
lasopsiD
-gnilcyceR-yrevoceR-esueR
laitnetop
LCA: Results
A1 A2 A3 A4 A5 B1 B2 B3 B4 B5 B6 B7 C1 C2 C3 C4 D
X X X X MND MND MND MND MND MND MND MND X X X X X
Core environmental impact indicators
Indicator Unit A1 A2 A3 A4 C1 C2 C3 C4 D
GWP-total kg CO2 eq. 3,29 E+01 1,8 E+00 6,91 E+00 3,15 E+00 0 3,47 E-01 0 9,86 E-04 -3,69 E+01
GWP-fossil kg CO2 eq. 3,30 E+01 1,8 E+00 5,91 E+00 3,14 E+00 0 3,46 E-01 0 9,83 E-04 -3,71 E+01
GWP-biogenic kg CO2 eq. -1,52 E-01 4,36 E-03 9,98 E-01 4,95 E-03 0 8,29 E-04 0 2,89 E-06 1,95 E-01
GWP-LULUC kg CO2 eq. 1,34 E-02 6,16 E-04 8,57 E-03 1,24 E-03 0 1,17 E-04 0 9,68 E-08 -1,37 E-02
ODP kg CFC11 eq. 2,05 E-06 4,08 E-07 1,35 E-06 7,30 E-07 0 7,86 E-08 0 1,35 E-10 -1,74 E-06
AP mol H⁺ eq. 1,25 E-01 5,00 E-03 3,92 E-02 3,89 E-02 0 1,39 E-03 0 6,57 E-05 -1,40 E-01
EP-freshwater kg P eq. 1,38 E-02 1,23 E-04 1,17 E-02 1,77 E-04 0 2,33 E-05 0 9,34 E-08 -1,62 E-02
EP-marine kg N eq. 3,07 E-02 1,04 E-03 6,57 E-03 9,56 E-03 0 4,25 E-04 0 3,13 E-05 -3,51 E-02
EP-terrestial mol N eq. 3,11 E-01 1,13 E-02 6,79 E-02 1,06 E-01 0 4,63 E-03 0 3,65 E-04 -3,55 E-01
POCP kg NMVOC eq. 1,49 E-01 4,33 E-03 1,12 E-02 1,91 E-02 0 1,42 E-03 0 9,58 E-05 -1,72 E-01
ADP-M&M kg Sb eq. 6,60 E-05 6,60 E-06 2,69 E-05 6,48 E-06 0 1,25 E-06 0 2,27 E-09 -4,96 E-05
ADP-fossil MJ 3,52 E+02 2,72 E+01 1,39 E+02 4,78 E+01 0 5,24 E+00 0 1,54 E-02 -3,63 E+02
WDP m³ 6,92 E+00 7,88 E-02 1,29 E-00 1,34 E-01 0 1,49 E-02 0 -3,58 E-03 -6,15 E+00
GWP-total: Global Warming Potential; GWP-fossil: Global Warming Potential fossil fuels; GWP-biogenic: Global Warming Potential biogenic; GWP-LULUC: Global
Warming Potential land use and land use change; ODP: Depletion potential of the stratospheric ozone layer; AP: Acidification potential, Accumulated Exceedance; EP-
freshwater: Eutrophication potential, fraction of nutrients reaching freshwater end compartment; See “additional Norwegian requirements” for indicator given as PO4
eq. EP-marine: Eutrophication potential, fraction of nutrients reaching freshwater end compartment; EP-terrestial: Eutrophication potential, Accumulated Exceedance;
POCP: Formation potential of tropospheric ozone; ADP-M&M: Abiotic depletion potential for non-fossil resources (minerals and metals); ADP-fossil: Abiotic depletion
potential for fossil resources; WDP: Water deprivation potential, deprivation weighted water counsumption
EPD for the best environmental decision 8
Additional environmental impact indicators
Indicator Unit A1 A2 A3 A4 C1 C2 C3 C4 D
PM Disease inc. 2,20 E-06 1,14 E-07 4,66 E-07 2,18 E-07 0 2,40 E-08 0 5,18 E-10 -2,56 E-06
IRP kBq U-235 eq 1,01 E+00 1,43 E-01 8,64 E-01 2,38 E-01 0 2,74 E-02 0 2,48 E-05 -9,98 E-01
ETP-fw CTUe 7,78 E+02 2,09 E+01 5,17 E+01 3,45 E+01 0 4,00 E+00 0 4,06 E-03 -8,65 E+02
HTP-c CTUh 1,70 E-07 7,43 E-10 2,57 E-08 1,43 E-09 0 1,43 E-10 0 6,70 E-11 -2,08 E-07
HTP-nc CTUh 6,47 E-07 2,04 E-08 2,95 E-08 3,24 E-08 0 4,07 E-09 0 6,75 E-12 -7,19 E-07
SQP Pt 1,47 E+02 1,90 E+01 3,93 E+01 4,22 E+01 0 3,61 E+00 0 3,59 E-03 -1,64 E+02
PM: Particulate matter emissions; IRP: Ionising radiation, human health; ETP-fw: Ecotoxicity (freshwater); ETP-c: Human toxicity, cancer effects; HTP-nc: Human
toxicity, non-cancer effects; SQP: Land use related impacts / soil quality
EPD for the best environmental decision 9
Classification of disclaimers to the declaration of core and additional environmental
impact indicators
ILCD
Indicator Disclaimer
classification
Global warming potential (GWP) None
ILCD type /
Depletion potential of the stratospheric ozone layer (ODP) None
level 1
Potential incidence of disease due to PM emissions (PM) None
Acidification potential, Accumulated Exceedance (AP) None
Eutrophication potential, Fraction of nutrients reaching freshwater end
None
compartment (EP-freshwater)
Eutrophication potential, Fraction of nutrients reaching marine end compartment
ILCD type / None
(EP-marine)
level 2
Eutrophication potential, Accumulated Exceedance (EP-terrestrial) None
Formation potential of tropospheric ozone (POCP) None
Potential Human exposure efficiency relative to U235 (IRP) 1
Abiotic depletion potential for non-fossil resources (ADP-minerals&metals) 2
Abiotic depletion potential for fossil resources (ADP-fossil) 2
Water (user) deprivation potential, deprivation-weighted water consumption
2
(WDP)
ILCD type /
Potential Comparative Toxic Unit for ecosystems (ETP-fw) 2
level 3
Potential Comparative Toxic Unit for humans (HTP-c) 2
Potential Comparative Toxic Unit for humans (HTP-nc) 2
Potential Soil quality index (SQP) 2
Disclaimer 1 – This impact category deals mainly with the eventual impact of low dose ionizing radiation on
human health of the nuclear fuel cycle. It does not consider effects due to
possible nuclear accidents, occupational exposure nor due to radioactive waste disposal in underground facilities.
Potential ionizing radiation from the soil, from radon and from some
construction materials is also not measured by this indicator.
Disclaimer 2 – The results of this environmental impact indicator shall be used with care as the uncertainties on
these results are high or as there is limited experienced with the indicator
EPD for the best environmental decision 10
Resource use
Indicator Unit A1 A2 A3 A4 C1 C2 C3 C4 D
RPEE MJ 7,63 E+00 2,71 E-01 3,02 E+01 3,75 E-01 0 5,14 E-02 0 1,21 E-04 -7,74 E+00
RPEM MJ 7,64 E+00 1,01 E-01 9,33 E+00 1,31 E-01 0 1,92 E-02 0 3,82 E-05 -6,66 E+00
TPE MJ 1,53 E+01 3,72 E-01 3,95 E+01 5,05 E-01 0 7,06 E-02 0 1,59 E-04 -1,44 E+01
NRPE MJ 3,52 E+02 2,72 E+01 1,40 E+02 4,78 E+01 0 5,24 E+00 0 1,54 E-02 -3,63 E+02
NRPM MJ 7,14 E-03 5,70 E-04 7,69 E-04 1,32 E-03 0 1,08 E-04 0 2,82 E-08 -7,03 E-03
TRPE MJ 3,52 E+02 2,72 E+01 1,40 E+02 4,78 E+01 0 5,24 E+00 0 1,54 E-02 -3,63 E+02
SM kg 3,8 E+00 0 0 0 0 0 0 0 0
RSF MJ 0 0 0 0 0 0 0 0 0
NRSF MJ 0 0 0 0 0 0 0 0 0
W m3 1,75 E-01 2,78 E-03 6,18 E-02 4,32 E-03 0 5,26 E-04 0 1,02 E-04 -1,56 E-01
RPEE Renewable primary energy resources used as energy carrier; RPEM Renewable primary energy resources used as raw materials; TPE Total use of renewable primary
energy resources; NRPE Non renewable primary energy resources used as energy carrier; NRPM Non renewable primary energy resources used as materials; TRPE Total
use of non renewable primary energy resources; SM Use of secondary materials; RSF Use of renewable secondary fuels; NRSF Use of non renewable secondary fuels; W Use
of net fresh water
End of life – Waste
Indicator Unit A1 A2 A3 A4 C1 C2 C3 C4 D
HW kg 2,47 E-03 7,11 E-05 1,06 E-05 9,59 E-05 0 1,36 E-05 0 2,12 E-08 -3,02 E-03
NHW kg 5,71 E+00 1,33 E+00 4,45 E-01 3,10 E+00 0 2,51 E-01 0 1,28 E-02 -6,80 E+00
RW kg 5,74 E-04 1,86 E-04 4,20 E-04 3,30 E-04 0 3,59 E-05 0 1,54 E-08 -6,17 E-04
HW Hazardous waste disposed; NHW Non hazardous waste disposed; RW Radioactive waste disposed
EPD for the best environmental decision 11
End of life – output flow
Indicator Unit A1 A2 A3 A4 C1 C2 C3 C4 D
CR kg 0 0 0 0 0 0 0 0 0
MR kg 0 0 1,23 E+00 0 0 0 0 3,61 E-01 1,95 E+01
MER kg 0 0 0 0 0 0 0 2,47 E-01 0
EEE MJ 0 0 0 0 0 0 0 3,43 E-01 0
ETE MJ 0 0 0 0 0 0 0 6,37 E-01 0
CR Components for reuse; MR Materials for recycling; MER Materials for energy recovery; EEE Exported electric energy; ETE Exported thermal energy
Reading example: 9,0 E-03 = 9,0*10-3 = 0,009
Information describing the biogenic carbon content at the factory gate
Biogenic carbon content Unit Value
Biogenic carbon content in product kg C 0
Biogenic carbon content in the accompanying packaging kg C 0,024
EPD for the best environmental decision 12
Additional Norwegian requirements
Greenhouse gas emission from the use of electricity in the manufacturing phase
National production mix from import, low voltage (production of transmission lines, in addition
to direct emissions and losses in grid) of applied electricity for the manufacturing prosess(A3).
National electricity grid Unit Value
Latvian electricity grid (from Ecoinvent 3.7.1.) kg CO2 -eq/kWh 0,416
Additional environmental impact indicators required in NPCR Part A for construction
products
In order to increase the transparency of biogenic carbon contribution to climate impact, the
indicator for GWP has been sub-divided into the following:
GWP-IOBC Climate impacts calculated according to the principle of instantanious oxidation
GWP-BC Climate impacts from the net uptake and emission of biogenic carbon from each module.
In addition, EP-freshwater shall also declared as PO4 eq.
Indicator Unit A1 A2 A3 A4 C1 C2 C3 C4 D
EP-
kg PO4 eq. 5,00 E-03 1,63 E-04 3,28 E-02 2,78 E-04 0 3,12 E-05 0 2,24 E-08 -5,23 E-03
freshwater*
GWP-IOBC kg CO2 eq. 3,31E+01 1,80E+00 5,91E+00 3,15E+00 0 3,46E-01 0 9,83E-04 -3,71E+01
GWP-BC kg CO2 eq. -1,52 E-01 4,36 E-03 9,98 E-01 4,95 E-03 0 8,29 E-04 0 2,89 E-06 1,95 E-01
GWP kg CO2 eq. 3,29 E+01 1,8 E+00 6,91 E+00 3,15 E+00 0 3,47 E-01 0 9,86 E-04 -3,69 E+01
EP-freshwater* Eutrophication potential, fraction of nutrients reaching freshwater end compartment.
Declared as PO4 eq. GWP-IOBC Global warming potential calculated according to the principle of
instantanious oxidation. GWP-BC Global warming potential from net uptake and emissions of biogenic carbon
from the materials in each module. GWP Global warming potential
Hazardous substances
The declaration is based upon reference to threshold values and/or test results and/or material
safety data sheets provided to EPD verifiers. Documentation available upon request to EPD
owner.
⊠ The product contains no substances given by the REACH Candidate list or the Norwegian
priority list.
□ The product contains substances given by the REACH Candidate list or the Norwegian
priority list that are less than 0,1 % by weight.
□ The product contain dangerous substances, more then 0,1% by weight, given by the
REACH Candidate List or the Norwegian Priority list, see table.
□ The product contains no substances given by the REACH Candidate list or the Norwegian
priority list. The product is classified as hazardous waste (Avfallsforskiften, Annex III), see
table.
Indoor environment
The product meets the requirements for low emissions.
Carbon footprint
Carbon footprint has not been worked out for the product.
EPD for the best environmental decision 13
Bibliography
ISO 14025:2010 Environmental labels and declarations - Type III
environmental declarations - Principles and procedures
ISO 14044:2006 Environmental management - Life cycle assessment -
Requirements and guidelines
EN 15804:2012+A2:2019 Sustainability of construction works - Environmental
product declaration - Core rules for the product category of
construction products
ISO 21930:2007 Sustainability in building construction - Environmental
declaration of building products
PEP-PCR-ed3-EN-2015 04 02. Product Category Rules for Electrical, Electronic and HVAC-
R Products
PSR-0011-ed1.0-EN-2018 02 09. Specific rules for hot water radiators or towel radiators
EN 442-1:2014 Radiators and convectors – Part 1. Technical specifications
and requirements
EN 442-2:2014 Radiators and convectors Test methods and rating
EN 13501 – 1 Fire classification of construction products and building
elements – Part 1: Classification using data from reaction to
fire tests
ISO 14040:2006 Environmental management – Life cycle assessment –
Principles and framework
ISO 14044:2006 Environmental management – Life cycle assessment –
Requirements and guidelines
UNI EN ISO 9001:2015 Quality management systems — Requirements
UNI EN ISO 14001:2015 Environmental management systems — Requirements
with guidance for use
ISO 50001:2018 Energy management systems — Requirements with
guidance for use
LCA software SimaPro 9.2
Program Operator tlf +47 23 08 80 00
The Norwegian EPD Foundation
Post Box 5250 Majorstuen, 0303 Oslo e-post: post@epd-norge.no
Norway web www.epd-norge.no
Publisher tlf +47 23 08 80 00
The Norwegian EPD Foundation
Post Box 5250 Majorstuen, 0303 Oslo e-post: post@epd-norge.no
Norway web www.epd-norge.no
Owner of the declaration tlf +371 29 47 47 39
Lyngson, SIA
Akaci, Olaines novadas, Olaines pagasts e-post: Uldis.Benhens@lyngson.lv
Latvia web www.lyngson.lv
Author of the life cycle assesment tlf +371 67 25 68 29
Bureau Veritas
Duntes ieal 17A, Ziemelu rajons, Riga, LV-1005 e-post: riga@lv.bureauveritas.com
Latvia web www.bureauveritas.lv
EPD for the best environmental decision 14
EPD for the best
environmental
decision
www.epd-norge.no
The Norwegian EPD foundation
