ver1 2015
ENVIRONMENTAL PRODUCT DECLARATION
in accordance with ISO 14025, ISO 21930 and EN 15804
Owner of the declaration: Hydro Aluminium AS
Program operator: The Norwegian EPD Foundation
Publisher: The Norwegian EPD Foundation
Declaration number: NEPD-2262-1034-EN
Registration number: NEPD-2262-1034-EN
ECO Platform reference number: -
Issue date: 18.06.2020
Valid to: 18.06.2025
Hydro Aluminium Sheet Ingot Products
Hydro Aluminium AS
www.epd-norge.no
NEPD-2262-1034-EN Hydro Aluminium Sheet Ingot Products
General information
Product: Owner of the declaration:
Hydro Aluminium Sheet Ingot Products Hydro Aluminium AS
Contact person: Stian Rørvik
Phone: +47 99 20 64 31
e-mail: stian.rorvik@hydro.com
Program operator: Manufacturer:
The Norwegian EPD Foundation Hydro Alumium AS
Pb. 5250 Majorstuen, 0303 Oslo Drammensveien 263, N-0240 Oslo
Phone: +47 97722020 Phone: +47 22538100
e-mail: post@epd-norge.no e-mail: greener@hydro.com
Declaration number: Place of production:
NEPD-2262-1034-EN Hydro Aluminium Hoyanger
Hydro Aluminium Aardal
ECO Platform reference number: Management system:
IATF 16949, ISO 9001:2016, ISO 14001,
ISO 45001, ISO 50001
This declaration is based on Product Category Rules: Organisation no:
CEN Standard EN 15804 serves as core PCR 917 537 534
NPCR 013, "Version 3.0 Part B for steel and aluminium
construction products"
Statement of liability: Issue date:
The owner of the declaration shall be liable for the 18.06.2020
underlying information and evidence. EPD Norway shall
not be liable with respect to manufacturerinformation, life Valid to:
cycle assessment data and evidences. 18.06.2025
Declared unit: Year of study:
1 kg Hydro Aluminium Sheet Ingot 2020
Declared unit with option: Comparability:
1 kg Hydro Aluminium Sheet Ingot, including waste handling EPD of construction products may not be comparable if they
and possible environmental benefits after end of life. not comply with EN 15804 and seen in a building context.
Functional unit: The EPD has been worked out by:
The product is an input to packaging (33%), the automotive Irmeline de Sadeleer, Andreas Brekke, Kari-Anne Lyng
industry (33%) and the buidling and construction industry
(33%). No use scerarios are defines, hence no functional unit.
Verification:
The CEN Norm EN 15804 serves as the core PCR.
Independent verification of the declaration and data, according
to ISO14025:2010
internal external
Approved
Third party verifier:
Jane Anderson
(Independent verifier approved by EPD Norway)
NEPD-2262-1034-EN Hydro Aluminium Sheet Ingot Products 2/8
Product
Product description: Technical data:
This EPD covers production of Sheet Ingot from Hydro Aluminium’ All products are produced according to European standard
s Norwegian Smelters. The primary Aluminum used in the EN-487 and according to customer requirements.
products is produced based on renewable power production in Sheet ingots are produced in thicknesses ranging from 400
Norway. Products covered are variants within the 1xxx, 3xxx, 600 mm, widths from 800 to 2200 mm and lengths up to 8.5
4xxx, 5xxx, 6xxx and 8xxx alloy groups. m
Weight between 2 and 30 mt
For more detailed information about shapes, dimensions
and tolerances:
https://www.hydro.com/en-NO/products-and-
Product specification: services/casthouse-products/sheet-ingots/
Materials kg %
Primary Liquid Al from own Electrolysis 0,86 86 % Market:
Primary Metal from external sources 0,12 12 % European Rolling Mills
Alloying elements 0,02 2 %
Reference service life, product:
Dependent on product application, but the material itself
Examples of Industry we serve: has an infinite life time.
Automotive, Packaging, Foil, B&C, General Engineering
Lithographic sheets & bright applications. Reference service life, building:
Dependent on product application, but the material itself has
an infinite life time.
NEPD-2262-1034-EN Hydro Aluminium Sheet Ingot Products 3/8
LCA: Calculation rules
Declared unit: System boundary:
1 kg Hydro Aluminium Sheet Ingot. The EPD also covers Cradle to gate with options. The following stages have been
modules C2-C4 and D. declared: A1-A4, C2-C4 and D. Further specified in flow
sheet below.
The Hydro Aluminium Sheet Ingots are produced in the
Norwegian smelters in Årdal and Høyanger. The presented Module D covers the potential benefits from recycling of
results is a weighed average of production volumes in 2018. Hydro Aluminium Foundry Alloy after end of useful life.
Module D covers all necessary stages from C3 until the
aluminium is back on the market and compares to the
environmental performance of an average market foundry
alloy. The module is further specified under scenarios.
Data quality: Cut-off criteria:
Specific data are used for all of Hydro's processes, based on the All major raw materials and all the essential energy is
production year 2018, and are collected the first months of 2019 included. The production process for raw materials and
and 2020. As Hydro has ownership in a total value chain from energy flows that are included with very small amounts
mining of bauxite to production of aluminium extrusion ingots, all (<1%) are not included. This cut-off rule does not apply for
stages from A1 to A4 are covered by specific data. Background hazardous materials and substances, and mostly apply for
data on for instance transport and electricity production are from alloying elements that are added in less than per
ecoinvent 3.4 (April 2018) thousandth.
Allocation:
The allocation is made in accordance with the provisions of EN
15804. Incoming energy and water and waste production inhouse
is allocated equally among all products through mass allocation.
For almost all processes, detailed data are provided for each
process step, and the main allocation is between aluminium
hydroxide and aluminium oxide in the production of alumina.
Effects of primary production of recycled materials are allocated to
the main product in which the material was used. The recycling
process and transportation of the material is allocated to this
analysis.
NEPD-2262-1034-EN Hydro Aluminium Sheet Ingot Products 4/8
LCA: Scenarios and additional technical information
The following information describe the scenarios in the different modules of the EPD.
The transport from production sites to market is assumed to be the weighted distance from the two smelters in Norway to a location
in central Europe, where 97% is transported to Rotterdam by ship and 3% are transported with truck. Of the 97%, 20% is
transported by train, 75% by barge, and the rest on truck.
Transport from production place to user (A4)
Type Capacity utilisation (incl. Type of vehicle Distance km Fuel/Energy
return) % consumption
Truck 50 Lorry, >32 metric tons, Euro V 585 2.46E-02 l/tkm
Boat 80 Cargo ship, 5000 tons 1129 1.56E-02 l/tkm
Barge 60 Freight, inland waterways, barge 230 1.13E-02 l/tkm
Train 50 Freight train 930 0.31 MJ/tkm
Most of the aluminium used for construction purposes is collected (approximately 96%) and recycled (approximately
97% of the collected aluminium), giving a total of 93% recycled. The rest is assumed landfilled. About 65% of the
aluminium used for food and packaging purposes is collected and recycled (approximately 97% of the collected
aluminium), giving a total of 62,3% recycled. The rest is assumed incinerated with energy recovery. Most of the
aluminium used in the automotive industry is collected (approximately 95%) and recycled (approximately 97% of the
collected aluminium), giving a total of 92% recycled. The rest is assumed landfilled.
End of Life (C2, C3, C4)
Unit Value
Hazardous waste disposed kg -
Collected as mixed construction waste kg 0.845
Reuse kg -
Recycling kg 0.818
Energy recovery kg 0.142
To landfill kg 0.029
*142 grams of the original 1 kg of aluminium is going to incineration. No loads or beneifts are attribuded to this flow.
Transport to waste processing (C2)
Type Capacity utilisation (incl. Type of vehicle Distance km Fuel/Energy
Truck 40 Lorry, >32 metric tons, Euro V 50 2.85E-02 l/tkm
Aluminium from construction site to waste handling site is assumed to be transported in an older medium-sized lorry with
smaller capacity utilization than in the production system
Benefits and loads beyond the system boundaries (D)
Unit Value
Aluminium sheet ingot to recycling g 822
Aluminium collected and recycled is assumed to replace an average extrusion ingot in Europe consisting of 40% recycled
and 60% primary aluminium. This is a conservative approach.
NEPD-2262-1034-EN Hydro Aluminium Sheet Ingot Products 5/8
LCA: Results
All results are calculated with the use of SimaPro v.9 (2019) and impact methods according to ISO 15804. Results are based on a
weighted average between three production sites.
System boundaries (X=included, MND= module not declared, MNR=module not relevant)
Environmental impact
Unit
1,03E+00
Resource use
1,75E-02
0,00E+00
1,75E-02 1,06E-03
1,02E+00 1,07E-01
0,00E+00 0,00E+00
1,02E+00 1,07E-01
0,00E+00 0,00E+00
0,00E+00
0,00E+00
slairetam
waR
ylbmessA
Product stage Assemby stage
A1 B6
C2
tropsnarT
B1
kg CO -eqv
2
AP
4,46E-04 -6,79E-03
1,46E-06
ADPE 1,11E-01
Parameter C2 D
5,95E+01
MJ 0,00E+00 0,00E+00
MJ 1,53E-01
1,38E+00
0,00E+00
TRPE MJ 4,58E+01 1,38E+00
0,00E+00
MJ 0,00E+00 0,00E+00 0,00E+00
MJ 0,00E+00 0,00E+00 0,00E+00
m3 1,47E-04 2,00E-05
tropsnarT
A2 B5 C1
x x MND MND MND MND
Parameter
4,65E+00 6,91E-03 -4,31E+00
POCP 1,14E-06
kg SO -eqv 2
0,00E+00
2,08E-08
MJ 4,48E+01 1,23E+00
GWP Global warming potential; ODP Depletion potential of the stratospheric ozone layer; POCP Formation potential of tropospheric
photochemical oxidants; AP Acidification potential of land and water; EP Eutrophication potential; ADPM Abiotic depletion potential for non fossil
resources; ADPE Abiotic depletion potential for fossil resources
RPEE MJ
RPEM
TPE
NRPM
ecnanetniaM
esu
retaw
lanoitarepO
A3 A4 A5 B2 B4
MND
gnirutcafunaM
B7
x
noitilomed
noitcurtsnoc-eD
Beyond the
system
boundaries
MND MND
NRPE
riapeR
tnemhsibrufeR
Use stage
MND
esu
ygrene
lanoitarepO
D
x
A1-A3 A4
GWP 2,22E-01
ODP kg CFC11-eqv 4,16E-07 1,20E-08
kg C H -eqv 2 4 1,46E-03 1,55E-05
2,70E-02 4,40E-04 2,71E-05
EP kg PO 43--eqv 6,40E-03 7,14E-05 6,36E-06
ADPM kg Sb-eqv 8,92E-06 2,59E-08
Unit A1-A3 C3
1,06E-03 1,53E-01 0,00E+00
0,00E+00 0,00E+00
5,95E+01 0,00E+00
MJ 4,58E+01 0,00E+00
MJ 0,00E+00 0,00E+00
0,00E+00
kg 0,00E+00
NRSF 0,00E+00
W -3,86E-02
RPEE Renewable primary energy resources used as energy carrier; RPEM Renewable primary energy resources used as raw materials; TPE
Total use of renewable primary energy resources; NRPE Non renewable primary energy resources used as energy carrier; NRPM Non
renewable primary energy resources used as materials; TRPE Total use of non renewable primary energy resources; SM Use of secondary
materials; RSF Use of renewable secondary fuels; NRSF Use of non renewable secondary fuels; W Use of net fresh water
lasopsiD
-yrevoceR-esueR laitnetop-gnilcyceR
C4
x
D
gnissecorp
etsaW
C2
x
tropsnarT
C3
x x
esU
B3
MND
C3 C4
3,44E-02
1,28E-09 8,89E-09 -2,64E-07
2,77E-05 0,00E+00 -2,31E-03
6,28E-04 -2,74E-02
0,00E+00 -1,08E-05
0,00E+00 -4,17E+01
C4
tnemecalpeR
End of life stage
0,00E+00
0,00E+00
0,00E+00
A4
-2,03E+01
0,00E+00
-2,03E+01
-5,07E+01
0,00E+00
-5,07E+01
SM 0,00E+00 0,00E+00
RSF 0,00E+00 0,00E+00 0,00E+00
0,00E+00
9,37E-02 0,00E+00
NEPD-2262-1034-EN Hydro Aluminium Sheet Ingot Products 6/8
End of life - Waste
Parameter Unit A1-A3 A4 C2 C3 C4 D
HW kg 2,09E-02 5,18E-07 6,76E-08 5,43E-03 0,00E+00 4,35E-03
NHW kg 3,37E+00 9,09E-03 5,65E-03 1,24E+00 5,94E-02 -2,20E+00
RW kg 1,87E-04 7,05E-06 7,21E-07 4,45E-06 0,00E+00 -2,00E-04
HW Hazardous waste disposed; NHW Non hazardous waste disposed; RW Radioactive waste disposed
End of life - Output flow
Parameter Unit A1-A3 A4 C2 C3 C4 D
CR kg - - - - - -
MR kg - - - 8,22E-01 - -
MER kg - - - 1,38E-01 - -
EEE MJ - - - - - -
ETE MJ - - - - - -
CR Components for reuse; MR Materials for recycling; MER Materials for energy recovery; EEE Exported electric energy; ETE Exported thermal
energy
Reading example: 9.0 E-03 = 9.0*10-3 = 0.009
Additional Norwegian requirements
Greenhouse gas emission from the use of electricity in the manufacturing phase
National production mix from import, low voltage (production of transmission lines, in addition to direct emissions and losses in grid)
of applied electricity for the manufacturing process (A3).
Data source Amount Unit
ecoinvent v3.4 (April 2018) 4 g CO -eq./kWh
2
Dangerous substances
The product contains no substances given by the REACH Candidate list or the Norwegian priority list
The product contains substances given by the REACH Candidate list or the Norwegian priority list that are less than 0.1 %
by weight.
The product contain dangerous substances, more than 0.1% by weight, given by the REACH Candidate List or the
Norwegian Priority list, see table.
The product contains no substances given by the REACH Candidate list or the Norwegian priority list. The product is
classified as hazardous waste (Avfallsforskiften, Annex III), see table.
Name CAS no. Amount
Indoor environment
Not relevant
Carbon footprint
Calculations connected to climate change and global warming potential (GWP) include greenhouse gas emissions from fossil
sources and land use change connected to extraction of bauxite, but does not include calculations of biogenic emissions of CO .
2
NEPD-2262-1034-EN Hydro Aluminium Sheet Ingot Products 7/8
Bibliography
ISO 14025:2010 Environmental labels and declarations - Type III environmental declarations - Principles and
procedures
ISO 14044:2006 Environmental management - Life cycle assessment - Requirements and guidelines
EN 15804:2012+A1:2013 Sustainability of construction works - Environmental product declaration - Core rules for the
product category of construction products
ISO 21930:2007 Sustainability in building construction - Environmental declaration of building products
NPCR 013 NPCR 013 version 3.0 Part B for steel and aluminium construction products.
Sadeleer, I., Brekke, A. and Background report for the Environmental Product Declarations for Hydro Aluminium Wire
Lyng, Kari-Anne (2020) Rod, Hydro Aluminium Sheet Ingot and Hydro Aluminium Foundry Alloy
Program operator Phone: +47 97722020
The Norwegian EPD Foundation
Post Box 5250 Majorstuen, 0303 Oslo e-mail: post@epd-norge.no
Norway web www.epd-norge.no
Publisher Phone: +47 97722020
The Norwegian EPD Foundation
Post Box 5250 Majorstuen, 0303 Oslo e-mail: post@epd-norge.no
Norway web www.epd-norge.no
Owner of the declaration Phone: +47 99 20 64 31
Hydro Aluminium AS Fax
Drammensveien 263 e-mail: stian.rorvik@hydro.com
N-0240 Oslo web www.hydro.com
Author of the Life Cycle Assessment Phone: +47 69 35 11 00
Østfoldforskning Fax +47 69 34 24 94
Company logo
Stadion 4 e-mail: post@ostfoldforskning.no
1671 Kråkerøy web www.ostfoldforskning.no
NEPD-2262-1034-EN Hydro Aluminium Sheet Ingot Products 8/8
