ver1 2015
ENVIRONMENTAL PRODUCT DECLARATION
in accordance with ISO 14025, ISO 21930 and EN 15804
Owner of the declaration: Fora Form AS
Program operator: The Norwegian EPD Foundation
Publisher: The Norwegian EPD Foundation
Declaration number: NEPD-3735-2683-EN
Registration number: NEPD-3735-2683-EN
ECO Platform reference number: -
Issue date: 22.09.2022
Valid to: 22.09.2027
Con II unpholstered - high back and armrest
Fora Form AS
www.epd-norge.no
NEPD-3735-2683-EN Con II unpholstered - high back and armrest
1 / 8
General information
Product: Owner of the declaration:
Con II unpholstered - high back and armrest
Fora Form AS
Contact person: Kåre Sætre
Phone: +47 700 46 000
e-mail: info@foraform.com
Program operator: Manufacturer:
Fora Form AS
The Norwegian EPD Foundation
Pb. 5250 Majorstuen, 0303 Oslo
Phone: +47 23 08 80 00
e-mail: post@epd-norge.no
Declaration number: Place of production:
Fora Form AS
NEPD-3735-2683-EN Mosflatevegen 6154 Ørsta
Norway
ECO Platform reference number: Management system:
NS-EN ISO 14001: 2015 No. 800406. NS-EN ISO 9001: 2015 No. 901268. NS-EN ISO
45001: 2018 No 907167.
This declaration is based on Product Category Rules: Organisation no:
986 581 421
CEN Standard EN 15804:2012+A1:2013 serves as core PCR
NPCR 026:2018 Part B for furniture
Statement of liability: Issue date: 22.09.2022
The owner of the declaration shall be liable for the underlying information and
evidence. EPD Norway shall not be liable with respect to manufacturer Valid to: 22.09.2027
information, life cycle assessment data and evidences.
Declared unit: Year of study:
1 Pcs Con II unpholstered - high back and armrest 2022
Declared unit with option: Comparability:
A1,A2,A3,A4,A5,B1,B2 EPDs from programmes other than the Norwegian EPD Foundation may not be
comparable
Functional unit: Development and verification of EPD:
Functional unit whitout cardboard / 8,79 kg The declaration has been developed and verified using EPD tool lca.tools
ver EPD2020.11, developed by LCA.no AS. The EPD tool is integrated into
the company's environmental management system, and has been
approved by EPD-Norway
General information on verification of EPD from EPD tools:
Independent verification of data, other environmental information and Developer of EPD:
the declaration according to ISO 14025:2010, § 8.1.3 and § 8.1.4. Individual
third party verification of each EPD is not required when the EPD tool is i) Kåre Sætre
integrated into the company's environmental management system, ii) the
procedures for use of the EPD tool are approved by EPDNorway, and iii) Reviewer of company-specific input data and EPD:
the proccess is reviewed annualy. See Appendix G of EPD-Norway's
General Programme Instructions for further information on EPD tools. Katrine Østgaard
Verification of EPD tool: Approved:
Independent third party verification of the EPD tool, background data
Sign
and test-EPD in accordance with EPDNorway's procedures and guidelines
for verification and approval of EPD tools.
Erik Svanes, Norsus AS
(no signature required) Håkon Hauan, CEO EPD-Norge
Key environmental indicators Unit Cradle to gate A1 - A3
Global warming kg CO2 eqv 52,19
Total energy use MJ 773,01
Amount of recycled materials % 33,84
NEPD-3735-2683-EN Con II unpholstered - high back and armrest
2 / 8
Product
Market: Technical data:
Furniture tested and approved
Worldwide
NS-EN 16139:2013
Product description:
Reference service life, product
Con is a versatile chair series for use in several areas of interaction, from
formal meeting rooms to canteens. Designer Lars Tornøe started out 15 years
with shell structures to design a "petite contribution" to Fora Form's
Reference service life, building
collection. The result has been a chair and bar stool made up of two
overlapping shells joined by a distinct button, a theme influenced by
Japanese armor. The layered design is the foundation for a series of
chairs with countless combination options with shells in different
designs, armrests and various bases.
Product specification
Con II, sled base - high back and armrest
Width: 55 cm
Height: 90 cm
Depth: 59 cm
Seat height: 46,5 cm
Weight: 8,79 kg
Recycled share in Recycled share in
Materials kg %
material (kg) material (%)
Metal - Aluminium 0,43 3,99 0,13 30,00
Metal - Steel 3,38 31,33 0,68 20,00
Textile - Wool 1,00 9,27 0,00 0,00
Plastic - Polyurethane (PUR) 1,00 9,27 0,00 0,00
Plastic - Acrylonitrile butadiene styrene (ABS) 0,18 1,67 0,00 0,00
Plastic - Polypropylene (PP) 2,60 24,10 1,30 50,00
Plastic - Polyoxymethylene (POM) 0,20 1,85 0,02 10,00
Cardboard 2,00 18,54 1,53 76,30
Total: 10,79 3,65
LCA: Calculation rules
Declared unit: Allocation:
The allocation is made in accordance with the provisions of EN 15804. Effects
1 Pcs Con II unpholstered - high back and armrest
of primary production of recycled materials is allocated to the main product
Cut-off criteria: in which the material was used. The recycling process and transportation of
the material is allocated to this analysis.
All major raw materials and all the essential energy is included. The
production processes for raw materials and energy flows with very small
amounts (less than 1%) are not included. These cut-off criteria do not
apply for hazardous materials and substances.
Data quality:
Specific data for the product composition are provided by the manufacturer. They represent the production of the declared product and were collected for
EPD development in the year of study. Background data is based on registered EPDs according to EN 15804, Ostfold Research databases, ecoinvent and other
LCA databases. The data quality of the raw materials in A1 is presented in the table below.
Materials Source Data quality Year
Plastic - Acrylonitrile butadiene styrene (ABS) ecoinvent 3.4 Database 2015
Plastic - Polypropylene (PP) ecoinvent 3.4 Database 2015
Plastic - Polyurethane (PUR) ecoinvent 3.4 Database 2015
Metal - Steel ecoinvent 3.3 Database 2016
Cardboard ecoinvent 3.4 Database 2017
Metal - Aluminium ecoinvent 3.4 Database 2017
Metal coating - Powder coating on steel ecoinvent 3.4 Database 2017
Plastic - Polyoxymethylene (POM) ecoinvent 3.4 Database 2017
Textile - Wool ecoinvent 3.4 Database 2017
Process ecoinvent 3.6 Database 2019
NEPD-3735-2683-EN Con II unpholstered - high back and armrest
3 / 8
System boundary:
Additional technical information:
We want you to enjoy your furniture for many years to come. If you follow our advice in this Quality and Maintenance Manual you contribute to prolonged
life of your furniture. We only use environmentally friendly materials and processes in our manufacturing unit in Ørsta Norway. Our goal is to manufacture
furniture that can last for generations. All furniture made by Fora Form are made of FSC certified wood, manufactured according to ISO 14001, and has an
EPD on all products. This ensures sustainability and a “cradle to cradle” philosophy. We actively work to reduce waste. All packing materials and waste are
being recycled according to Norsk Gjenvinning.
Norwegian and Swedish Møbelfakta are accredited test facilities where furniture quality, strength, durability, flammability, safety, emissions and materials are
tested and documented. A piece of furniture, which lives up to the three areas of requirements of Møbelfakta, has undergone extensive testing, is produced
according to ethical guidelines and has been approved according to environmental requirements. Møbelfakta is a guarantee of high quality products. Almost
all of Fora Forms collection is Møbelfakta approved.
Fora Form are ISO 9001 quality management, ISO 14001 environmental management and ISO 45001 occupational health and safety management certified.
Sustainability is important for Fora Form.
We continuously work to sort and reduce our waste, and collaborate with Norsk Gjenvinning and Grønt Punkt (Green Dot Norway plc) regarding recycling of
used packing materials. All wood is FSC certified.
Our manufacturing unit in Ørsta use electricity that is 100% originated from renewable sources.
Transportation to an average customer in Oslo is 540 km (A4: average European lorry > 32 tonnes)
NEPD-3735-2683-EN Con II unpholstered - high back and armrest
4 / 8
LCA: Scenarios and additional technical information
The following information describe the scenarios in the different modules of the EPD.
Transport from production place to user (A4)
Capacity utilisation Fuel/Energy
Type Type of vehicle Distance km Unit Value (l/t)
(incl. return) % consumption
Truck 38,8 % Truck, 16-32 tonnes, EURO 5 540 0,044606 l/tkm 24,09
Railway l/tkm
Boat l/tkm
Other Transportation l/tkm
Assembly (A5) Use (B1)
. Unit Value . Unit Value
Auxiliary kg Water (L) L/DU 1,00
Water consumption m3
Electricity consumption kWh
Other energy carriers MJ
Material loss kg
Output materials from waste treatment kg 2,0000
Dust in the air kg
VOC emissions kg
NEPD-3735-2683-EN Con II unpholstered - high back and armrest
5 / 8
LCA: Results
The LCA results are presented below for the declared unit defined on page 2 of the EPD document.
System boundaries (X=included, MND=module not declared, MNR=module not relevant)
Construction Beyond the
Product stage installation User stage End of life stage . system
stage bondaries
A1 A2 A3 A4 A5 B1 B2 B3 B4 B5 B6 B7 C1 C2 C3 C4 . D
X X X X X X X .
Environmental impact
Parameter Unit A1 A2 A3 A4 A5 B1 B2
GWP kg CO 2 -eq 5,16E+01 5,94E-01 3,94E-03 7,72E-01 1,07E+00 3,64E-04 0
ODP kg CFC11 -eq 2,37E-06 1,09E-07 4,11E-10 1,42E-07 1,25E-08 3,50E-11 0
POCP kg C 2H 4-eq 1,61E-02 1,13E-04 4,92E-06 1,26E-04 5,80E-05 1,16E-07 0
AP kg SO 2 -eq 3,09E-01 2,46E-03 2,35E-05 2,46E-03 5,40E-04 1,90E-06 0
EP kg PO 3- -eq 5,54E-02 3,55E-04 7,10E-06 4,08E-04 3,26E-04 2,39E-07 0
4
ADPM kg Sb -eq 1,80E-04 1,72E-06 1,83E-08 2,35E-06 1,63E-07 1,33E-09 0
ADPE MJ 5,27E+02 8,90E+00 4,61E-02 1,16E+01 1,09E+00 4,00E-03 0
GWP Global warming potential; ODP Depletion potential of the stratospheric ozone layer; POCP Formation potential of tropospheric photochemical oxidants;
AP Acidification potential of land and water; EP Eutrophication potential; ADPM Abiotic depletion potential for non fossil resources; ADPE Abiotic depletion
potential for fossil resources
Reading example: 9,0 E-03 = 9,0*10-3 = 0,009
*INA Indicator Not Assessed
waR slairetam tropsnarT gnirutcafunaM tropsnarT ylbmessA esU ecnanetniaM riapeR tnemecalpeR tnemhsibrufeR lanoitarepO ygrene esu lanoitarepO esu
retaw
-eD noitcurtsnoc noitilomed tropsnarT etsaW gnissecorp lasopsiD -yrevoceR-esueR -gnilcyceR laitnetop
NEPD-3735-2683-EN Con II unpholstered - high back and armrest
6 / 8
Resource use
Parameter Unit A1 A2 A3 A4 A5 B1 B2
RPEE MJ 1,02E+02 1,34E-01 3,01E-01 1,70E-01 1,20E+01 7,60E-04 0
RPEM MJ 3,16E+01 0,00E+00 0,00E+00 0,00E+00 0,00E+00 0,00E+00 0
TPE MJ 1,34E+02 1,34E-01 3,01E-01 1,70E-01 1,20E+01 7,60E-04 0
NRPE MJ 6,61E+02 9,12E+00 5,54E-02 1,19E+01 9,08E+00 6,14E-03 0
NRPM MJ 8,77E+01 0,00E+00 0,00E+00 0,00E+00 0,00E+00 0,00E+00 0
TRPE MJ 7,49E+02 9,12E+00 5,54E-02 1,19E+01 9,08E+00 6,14E-03 0
SM kg 3,65E+00 0,00E+00 0,00E+00 0,00E+00 0,00E+00 0,00E+00 0
RSF MJ 0,00E+00 0,00E+00 2,13E-05 0,00E+00 0,00E+00 0,00E+00 0
NRSF MJ 0,00E+00 0,00E+00 2,18E-02 0,00E+00 0,00E+00 0,00E+00 0
W m3 4,15E-01 1,69E-03 3,24E-05 2,23E-03 2,91E-03 1,17E-03 0
RPEE Renewable primary energy resources used as energy carrier; RPEM Renewable primary energy resources used as raw materials; TPE Total use of renewable
primary energy resources; NRPE Non renewable primary energy resources used as energy carrier; NRPM Non renewable primary energy resources used as
materials; TRPE Total use of non renewable primary energy resources; SM Use of secondary materials; RSF Use of renewable secondary fuels; NRSF Use of non
renewable secondary fuels; W Use of net fresh water
Reading example: 9,0 E-03 = 9,0*10-3 = 0,009
*INA Indicator Not Assessed
End of life - Waste
Parameter Unit A1 A2 A3 A4 A5 B1 B2
HW kg 2,49E-03 5,33E-06 7,29E-08 6,95E-06 2,32E-06 1,58E-08 0
NHW kg 3,29E+01 4,61E-01 2,26E-03 6,27E-01 7,99E-01 2,30E-04 0
RW kg INA* INA* INA* INA* INA* INA* 0
HW Hazardous waste disposed; NHW Non hazardous waste disposed; RW Radioactive waste disposed
Reading example: 9,0 E-03 = 9,0*10-3 = 0,009
*INA Indicator Not Assessed
End of life - Output flow
Parameter Unit A1 A2 A3 A4 A5 B1 B2
CR kg 0,00E+00 0,00E+00 0,00E+00 0,00E+00 0,00E+00 0,00E+00 0
MR kg 0,00E+00 0,00E+00 0,00E+00 0,00E+00 1,89E-02 0,00E+00 0
MER kg 0,00E+00 0,00E+00 0,00E+00 0,00E+00 0,00E+00 0,00E+00 0
EEE MJ INA* INA* INA* INA* INA* INA* 0
ETE MJ INA* INA* INA* INA* INA* INA* 0
CR Components for reuse; MR Materials for recycling; MER Materials for energy recovery; EEE Exported electric energy; ETE Exported thermal energy
Reading example: 9,0 E-03 = 9,0*10-3 = 0,009
*INA Indicator Not Assessed
NEPD-3735-2683-EN Con II unpholstered - high back and armrest
7 / 8
Additional Norwegian requirements
Greenhouse gas emissions from the use of electricity in the manufacturing phase
National production mix from import, low voltage (production of transmission lines, in addition to direct emissions and losses in grid) of applied electricity for the manufacturing
process (A3).
Electricity mix Data source Amount Unit
Energy, district heating, Norwegian average (kWh) Østfoldforskning 19,71 g CO2-ekv/kWh
Dangerous substances
The product contains no substances given by the REACH Candidate list or the Norwegian priority list.
Indoor environment
Our furniture doesn't contain any substanses that effect indoor clima
Additional environmental information
Key environmental indicators for variants for this EPD: Cradle to Gate analyse from A1 to A3
Global warming (kg Share of recycled
Variant number Total energy use (MJ)
CO2) material in product(%)
Con II - unpholstered - high backrest 44,94 700,87 34,94
Con II - low veneer backrest 32,46 535,95 33,91
Bibliography
ISO 14025:2010 Environmental labels and declarations - Type III environmental declarations - Principles and procedures.
ISO 14044:2006 Environmental management - Life cycle assessment - Requirements and guidelines.
EN 15804:2012+A1:2013 Environmental product declaration - Core rules for the product category of construction products.
ISO 21930:2017 Sustainability in buildings and civil engineering works - Core rules for environmental product declarations of construction products.
ecoinvent v3, Allocation, cut-off by classification, Swiss Centre of Life Cycle Inventories.
Iversen et al., (2018) eEPD v3.0 - Background information for EPD generator system. LCA.no report number 04.18
Vold et al., (2019) EPD generator for Norsk Industri, Background information for industry application and LCA data, LCA.no report number 06.19.
NPCR Part A: Construction products and services. Ver. 1.0. April 2017, EPD-Norge.
NPCR 026 Part B for Furniture. Ver. 2.0 October 2018, EPD-Norge.
Program operator and publisher Phone: +47 23 08 80 00
The Norwegian EPD Foundation e-mail: post@epd-norge.no
Post Box 5250 Majorstuen, 0303 Oslo,Norway web: www.epd-norge.no
Owner of the declaration Phone: +47 700 46 000
Fora Form AS e-mail: info@foraform.com
Mosflatevegen 6154 Ørsta web: www.foraform.no
Author of the Life Cycle Assessment Phone: +47 916 50 916
LCA.no AS e-mail: post@lca.no
Dokka 6B 1671 Kråkerøy web: www.lca.no
Developer of EPD generator Phone: +47 916 50 916
LCA.no AS e-mail: post@lca.no
Dokka 1C 1671 Kråkerøy web: www.lca.no
NEPD-3735-2683-EN Con II unpholstered - high back and armrest
8 / 8
