1114 NEPD
Ver. 2 2015(17)
ENVIRONMENTAL PRODUCT DECLARATION
in accordance with ISO 14025, ISO 21930 and EN 15804
Owner of the declaration: NorDan As
Program operator: The Norwegian EPD Foundation
Publisher: The Norwegian EPD Foundation
Declaration and registration number: NEPD-2389-1125-EN
ECO Platform registration number: -
Issue date: 23.09.2020
Valid to: 23.09.2025
NorDan NTech Villa Balcony door (security) - TE 105/80 (Without
aluminium cladding)
NorDan As
Owner of the declaration
www.epd-norge.no
NEPD-2389-1125-EN NorDan NTech Villa Balcony door (security) - TE 105/80 (Without aluminium cladding)
General information
Product: Owner of the declaration:
NorDan NTech Villa Balcony door (security) - TE 105/80 NorDan AS
(Without aluminium cladding) Kontaktperson: Fredrik Jonsson
Tlf: +46 (0) 10-130 01 78
e-post: fredrik.jonsson@nordan.se
Program holder: Manufacturer:
The Norwegian EPD Foundation NorDan sp. z o.o.
Post Box 5250 Majorstuen, 0303 Oslo Fabryczna 16, PL-64-200 Wolsztyn, Poland
Tlf: +47 977 22 020
e-mail: post@epd-norge.no Phone: +48 68 34 70 500
Fax: 048 68 34 73 541
Declaration number: Place of production:
NEPD-2389-1125-EN Powodowo, Poland
ECO Platform registration number: Management system:
NorDan sp. z o.o. Works with EN ISO 9001:2015, ISO
14001:2015
This declaration is based on Product Category Rules:
CEN Standard EN 15804 serves as core PCR NPCR014:2019
version 3.0 for Windows and doors Org. no.:
NO 979 776 233 MVA
Declaration of responsibility: Issue date:
The owner of the declaration shall be responsible for the 23.09.2020
underlying information and evidence. EPD Norway shall not
be responsible with regard to manufacturer information, life
cycle data and evidence.
Valid to:
23.09.2025
Declared unit: Year of study:
2020
Declared unit with option: Comparability:
EPD of construction products may not be comparable if they
are not comply with NS-EN 15804 and seen in a building
context.
Functional unit:
1 door set measuring 1.23 m x 2.18 m (reference door based
on EN 14351-1) with an essential parameter U-value = 0,84 The EPD has been worked out by:
and with an expected service life of 40 years. Roja Modaresi
Norsk Treteknisk Institutt
Verification:
Independent verification of the declaration and data,
according to ISO14025:2010
internal external
Approved
Third party verifier:
signiture
Clara Valente, Research scientist, Norsus
(Independent verifier approved by EPD Norway)
NEPD-2389-1125-EN NorDan NTech Villa Balcony door (security) - TE 105/80 (Without aluminium cladding)
2/9
Product
Product description: Technical data:
Door for use in exterior walls of domestic and commercial Security balcony door. Triple glazed, 105mm frame, 80mm
buildings. sash. Uwin 0,84W/m2K. Certified: BBA, Secured by Design,
SP Sitac “P”.
The total weight of the product is 93.17 kg. The packaging
has a average weight of 4.43 kg.
Product specification:
25% of aluminium and 18% of glass is produced from recycled
material. Market:
Europe, but scenarios beyond cradle to gate are based
on the situation in the Norwegian market.
Materialer kg %
Pine timber 25.38 27.24
Heat treated timber 0.44 0.47
Glass 56.92 61.09
Triple glazed Spacer 0.91 0.98
unit Butyl 0.06 0.06 Reference service life:
Sealant 1.35 1.45 The reference service life is 40 years for painted timber
Paint 0.72 0.77 frame
Aluminium 2.32 2.49
Plastic 0.17 0.18
Gasket 0.66 0.71
Metal- Steel alloys 4.07 4.37
Sealant and Glue 0.17 0.18
Total weight of the product 93.17 100
Wood packaging 4.2
Steel packaging 0.063
Plastic packaging 0.10
Paper, cardboard packaging 0.07
Total weight with packaging 97.60
LCA: Calculation rules
Functional unit: System boundary:
1 door set measuring 1.23 m x 2.18 m (reference door based All modules are included. Below is a technical flowchart for
on EN 14351-1) with an essential parameter U-value = 0,84 the production line at Nordan. Modul D is calculated with
and with an expected service life of 40 years. energy substitution and explained in the scenarios.
NEPD-2389-1125-EN NorDan NTech Villa Balcony door (security) - TE 105/80 (Without aluminium cladding)
3/9
Data quality Cut-off criteria:
Data is representative of year 2018 and was collected in 2019- All raw materails and energy use is included. Where data
2020. Data is taken from processes from Ecoinvent 3.1-3.5. Some was available for infrastructure from Ecoinvent, it is included.
processes are based on Ecoinvent v3.1 (2014) and v3.2 (2015), Example: ‘Metal working factory'. In the production process,
but all upstream processes are v3.4 (2017). Remaining data is raw materials and energy of low amounts are not included
based on Ecoinvent v3.5 (2018). "Allocation cut-off by (<1%). These cut-off rules do not apply to dangerous
classification" (2017) adjusted to improve representativeness. substances.
Allocation: Calculations of biogenic carbon:
Allocation is done in accordance with the provisions of EN 15804. Sequestration and release of biogenic carbon is included
Allocation of energy, water and waste from production is calculated according to EN 16485:2014. This is based on the modularity
by a physical allocation factor based on the manufacturer input. principle in EN 15804:2012 that specifies that the emissions
For waste produced at the manufacturing, the burdens for reuse, shall be accounted in the module that they occur. The
recycling and recovery is allocated by using this allocation factor. amount of carbon dioxide sequestrated is calulated in
accordance to EN 16449:2014. Timber comes from
sustainable forestry and has FSC certified traceability.
LCA: Scenarios and additional technical information
The following information describe the scenarios in the different modules of the EPD
The transportation from production to construction site is based on a scenario where the product is transported on a large lorry from
Poland to Oslo, Norway (1250 km) and then to a warehouse which is assumed to be in a 250 km radius from Oslo. Transport from
warehouse to a construction site is assumed to be 50 km on a medium truck.
Transport from production place to assembly/user (A4)
Type Capacity utilisation Type of vehicle Distance km Fuel/Energy Fuel/Energy
(incl. return) % consumption pr tkm consumption pr km
Truck 53 EURO5, >32 tonn 1500 0.023 l/tkm 0.31 l/km
Truck 26 EURO5, 16-32 tonn 50 0.045 l/tkm 0.25 l/km
Installation (A5)
Unit Value According to the report from EPD-Norge ‘Harmonising the
Auxiliary kg 0 documentation of scenarios beyond cradle to gate, EN 15804’ there is
Water consumption m3 0 no loss on site during construction activities. The window products in
Electricity consumption MJ 0 this EPD are painted and surface treated in the production and not at
Other energy carriers MJ 0 the building site. Therefore, there is only 2 items left in this module. 1)
Material loss kg 0 Waste treatment of packaging which is considered in the EPD
Output materials from waste treatment kg 4.43 calculations. 1) Energy use during installation. This can be varied
Dust in the air kg 0 depending on the floor, type of building and several other unknown
parameters, and therefore ignored in the calculation.
Maintenance (B2)/Repair (B3)
The maintenance scenario included cleaning, painting and change of
Unit Value IGU. Cleaning is performed three times per year. It is calculated with
1,5 dl of detergent and 3 litres of water each year. Windows without
Detergents kg 6
aluminium cladding are painted 2 times from inside and 4 times from
Water consumption l 120
outside. It is assumed that 5 gr of lubricating oil is used every year for
Lubricating oil kg 0.20
fittings and moving parts. No repair is assumed during the product
Paint kg 1.99
lifetime.
Transport tkm 2.45
Glazing unit kg 0
Synthetic rubber kg 0
Transport (IGU) tkm 0
NEPD-2389-1125-EN NorDan NTech Villa Balcony door (security) - TE 105/80 (Without aluminium cladding)
4/9
Replacement (B4)/Refurbishment (B5)
*Number or RSL (Reference Service Life). The window has RSL of
Unit Value 40 years for without aluminium cladding. Windows with 40 years RSL
Replacement cycle* yr 30 is assumed to have one entire window replacement during the lifetime
Electricity consumption kWh 0 of the building. It is assumed that this change is occured after 30
Replacement of worn parts 0 0 years when the IGU reaches its end of life. There is no need for
refurbishment during the product lifetime.
(C1) As there are no data for de-construction, it is assumed no activites in C1 in this study. The windows are assumed to be treated as
mixed waste and sent to incineration. The combustible materials are then energy recovered, while glass is assumed to end up in the
bottom ash and then landfilled. The metals are usually sorted out of the bottom ash and then recycled, but there is no data of the share
which are recycled and therefore standard values from Ecoinvent is utilized.
The transport of window as waste is calculated based on a scenario with 50 km distance.
Transport to waste processing (C2)
Type Capacity utilisation Type of vehicle Distance km Fuel/Energy Fuel/Energy
(incl. return) % consumption pr tkm consumption pr km
Truck 44 Unspecified 50 0.03l/tkm 0.28 l/km
Windows are assumed to be sorted as mixed construction waste and treated with incineration with energy recovery. However, The
manufacturer has documented the recycling potentials for its product in the Construction Product Declaration eBVD.
NorDan TE Dörr Trä 105, ID: C-SE556294452901-71
URL: https://www.ebvd.org/BMI/Document/Export/3054/0/Pdf
In the documentation, Chapter 10, the specific material recovery, and energy recovery potential is reported for the product.
End of Life (C1, C3, C4)
Unit Value
Hazardous waste disposed kg 0
Collected as mixed construction waste kg 93.17
Reuse kg 0
Recycling kg 2.96
Energy recovery kg 90.21
To landfill kg 0.00
The benefits beyond life cycle has been modelled based on the output flows from module C3. This includes energy from incineration
and scrap metal recovered from the ashes. The amount recovered metal is assumed to avoid production of primary metals in
accordance to 6.4.3.3 in EN 15804. The exported energy is substituting Norwegian district heating mix and electricity mix. Inventory
processes causing substitution of avoided virgin raw materials has be constructed for each material.
Benefits and loads beyond the system boundaries (D)
Unit Value
Substitution of electricity MJ 31.3
Substitution of thermal energy MJ 320.9
Substitution of raw materials kg 3.0
NEPD-2389-1125-EN NorDan NTech Villa Balcony door (security) - TE 105/80 (Without aluminium cladding)
5/9
LCA: Results
System boundaries (X = included)
X X X X X X X X X X
Environmental impact Without alu clad
Parameter Unit A1-A3 A4 A5 B1 B2 B3 B4 B5
GWP kg CO -ekv 1.41E+02 1.28E+01 6.29E+00 0.00E+00 12.2332 0.00E+00 2.14E+02 0.00E+00
2
ODP kg CFC11-ekv 8.31E-06 2.55E-06 0.00E+00 0.00E+00 9.55E-07 0.00E+00 1.12E-05 0.00E+00
POCP kg C H -ekv 2.27E-01 2.02E-03 0.00E+00 0.00E+00 0.006238 0.00E+00 2.29E-01 0.00E+00
2 4
AP kg SO -ekv 9.25E-01 3.47E-02 0.00E+00 0.00E+00 0.087845 0.00E+00 9.72E-01 0.00E+00
2
EP kg PO 3--ekv 1.26E-01 4.86E-03 0.00E+00 0.00E+00 0.009254 0.00E+00 1.34E-01 0.00E+00
4
EP kg PO 3--ekv 0.00E+00 0.00E+00 0.00E+00 4.11E-04 2.01E-03 7.35E-04 -1.24E-02
4
ADPM kg Sb-ekv 0.00E+00 0.00E+00 0.00E+00 1.67E-06 1.48E-06 -5.03E-05
-2.27E+02
noitcurtsnoc-eD
noitilomed tropsnarT
gnissecorp
etsaW
lasopsiD
-yrevoceR-esueR laitnetop
gnilcyceR
A1 A2 A3 A4 A5 B1 B2 B3 B4
gnirutcafunaM
tropsnarT
noitallatsni
noitcurtsnoC
egats esU
ecnanetniaM
riapeR
tnemecalpeR tnemhsibrufeR
esu
ygrene
lanoitarepO
Global warming potential in A1-A3 includes sequestration of 41.2 kg CO2 as carbon in the wood. This amount is accounted as an
emission in module C3. Additionally, it is included sequestration og 6.3 kg in the wood packaging. This is accounted as an emission
in module A5. The flow of biogenic carbon for the system is presented in page 9.
Construction Beyond the
Product stage and installation Use stage End of Life stage system
stage boundaries
B5 D
slairetam
waR
tropsnarT
esu
retaw
lanoitarepO
B6 B7 C1 C2 C3 C4
X X X X X X X
ADPM kg Sb-ekv 1.15E-03 2.59E-05 0.00E+00 0.00E+00 7.13E-05 0.00E+00 1.18E-03 0.00E+00
ADPE MJ 2.37E+03 2.22E+02 0.00E+00 0.00E+00 212.1657 0.00E+00 2.74E+03 0.00E+00
Parameter Unit B6 B7 C1 C2 C3 C4 D
GWP kg CO -ekv 0.00E+00 0.00E+00 0.00E+00 5.89E-01 5.23E+01 7.09E-01 -2.20E+01
2
ODP kg CFC11-ekv 0.00E+00 0.00E+00 0.00E+00 1.11E-07 6.36E-08 1.89E-07 -8.71E-07
POCP kg C H -ekv 0.00E+00 0.00E+00 0.00E+00 9.75E-05 3.76E-04 1.63E-04 -9.57E-03
2 4
AP kg SO -ekv 0.00E+00 0.00E+00 0.00E+00 2.30E-03 6.17E-03 3.98E-03 -1.18E-01
2
1.42E-06
ADPE MJ 0.00E+00 0.00E+00 0.00E+00 9.70E+00 1.16E+02 1.81E+01
GWP Global warming potential; ODP Depletion potential of the stratospheric ozone layer; POCP Formation potential of tropospheric
photochemical oxidants; AP Acidification potential of land and water; EP Eutrophication potential; ADPM Abiotic depletion potential for non fossil
resources; ADPE Abiotic depletion potential for fossil resources.
NEPD-2389-1125-EN NorDan NTech Villa Balcony door (security) - TE 105/80 (Without aluminium cladding)
6/9
Resource use without alu clad
Parameter Unit A1-A3 A4 A5 B1 B2 B3 B4 B5
RPEE MJ 8.37E+02 2.2E+00 0.00E+00 0.00E+00 2.88E+01 0.00E+00 1.27E+03 0.00E+00
RPEM MJ 5.21E+02 0.0E+00 0.00E+00 0.00E+00 0.00E+00 0.00E+00 8.98E+01 0.00E+00
TPE MJ 1.36E+03 2.2E+00 0.00E+00 0.00E+00 2.88E+01 0.00E+00 1.36E+03 0.00E+00
NRPE MJ 2.58E+03 2.3E+02 0.00E+00 0.00E+00 2.35E+02 0.00E+00 2.95E+03 0.00E+00
NRPM MJ 1.62E+02 0.0E+00 0.00E+00 0.00E+00 1.11E+01 0.00E+00 5.26E+01 0.00E+00
TRPE MJ 2.74E+03 2.3E+02 0.00E+00 0.00E+00 2.47E+02 0.00E+00 3.00E+03 0.00E+00
SM kg 7.30E-01 0.0E+00 0.00E+00 0.00E+00 0.00E+00 0.00E+00 7.30E-01 0.00E+00
RSF MJ 3.65E-01 0.0E+00 0.00E+00 0.00E+00 9.19E-03 0.00E+00 1.09E+00 0.00E+00
NRSF MJ 3.52E-01 0.0E+00 0.00E+00 0.00E+00 6.12E-03 0.00E+00 8.35E-01 0.00E+00
W m3 2.39E+01 3.9E-02 0.00E+00 0.00E+00 3.25E-01 0.00E+00 2.40E+01 0.00E+00
Resource use without alu clad
Parameter Unit B6 B7 C1 C2 C3 C4 D
RPEE MJ 0.0E+00 0.0E+00 0.0E+00 9.9E-02 4.3E+02 2.6E-01 -2.0E+02
RPEM MJ 0.0E+00 0.0E+00 0.0E+00 0.0E+00 -4.3E+02 0.0E+00 0.0E+00
TPE MJ 0.0E+00 0.0E+00 0.0E+00 9.9E-02 1.0E+00 2.6E-01 -2.0E+02
NRPE MJ 0.0E+00 0.0E+00 0.0E+00 9.9E+00 1.2E+02 1.9E+01 -2.4E+02
NRPM MJ 0.0E+00 0.0E+00 0.0E+00 0.0E+00 -1.1E+02 0.0E+00 0.0E+00
TRPE MJ 0.0E+00 0.0E+00 0.0E+00 9.9E+00 7.0E+00 1.9E+01 -2.4E+02
SM kg 0.0E+00 0.0E+00 0.0E+00 0.0E+00 0.0E+00 0.0E+00 0.0E+00
RSF MJ 0.0E+00 0.0E+00 0.0E+00 0.0E+00 7.2E-01 0.0E+00 -1.2E+02
NRSF MJ 0.0E+00 0.0E+00 0.0E+00 0.0E+00 4.8E-01 0.0E+00 -8.3E+01
W m3 0.0E+00 0.0E+00 0.0E+00 1.6E-03 1.9E-02 1.6E-02 -7.3E-01
RPEE Renewable primary energy resources used as energy carrier; RPEM Renewable primary energy resources used as raw materials; TPE
Total use of renewable primary energy resources; NRPE Non renewable primary energy resources used as energy carrier; NRPM Non
renewable primary energy resources used as materials; TRPE Total use of non renewable primary energy resources; SM Use of secondary
materials; RSF Use of renewable secondary fuels; NRSF Use of non renewable secondary fuels; W Use of net fresh water.
End of life-Waste without alu clad
Parameter Unit A1-A3 A4 A5 B1 B2 B3 B4 B5
HW kg 3.25E+00 1.37E-02 0.00E+00 0.00E+00 2.98E-02 0.00E+00 7.10E+01 0.00E+00
NHW kg 4.18E+01 1.76E+01 0.00E+00 0.00E+00 3.52E+00 0.00E+00 6.07E+01 0.00E+00
RW kg 2.80E-02 1.44E-03 0.00E+00 0.00E+00 5.01E-04 0.00E+00 2.96E-02 0.00E+00
End of life-Waste without alu clad
Parameter Unit B6 B7 C1 C2 C3 C4 D
HW kg 0.00E+00 0.00E+00 0.00E+00 6.88E-04 7.99E-03 6.77E+01 -1.18E-01
NHW kg 0.00E+00 0.00E+00 0.00E+00 5.77E-01 2.04E-01 5.45E-01 -3.53E+00
RW kg 0.00E+00 0.00E+00 0.00E+00 6.26E-05 2.27E-05 1.08E-04 -3.91E-04
HW Hazardous waste disposed; NHW Non hazardous waste disposed; RW Radioactive waste disposed
End of life- Output flow without alu clad
Parameter Unit A1-A3 A4 A5 B1 B2 B3 B4 B5
CR kg 0.00E+00 0.00E+00 0.00E+00 0.00E+00 0.00E+00 0.00E+00 0.00E+00 0.00E+00
MR kg 1.04E+00 0.00E+00 3.17E-01 0.00E+00 0.00E+00 0.00E+00 4.32E+00 0.00E+00
MER kg 5.91E-04 0.00E+00 4.21E+00 0.00E+00 0.00E+00 0.00E+00 4.21E+00 0.00E+00
EEE MJ 9.20E+00 0.00E+00 0.00E+00 0.00E+00 0.00E+00 0.00E+00 5.39E+01 0.00E+00
ETE MJ 1.01E+02 0.00E+00 0.00E+00 0.00E+00 0.00E+00 0.00E+00 4.10E+02 0.00E+00
End of life- Output flow without alu clad
Parameter Unit B6 B7 C1 C2 C3 C4 D
CR kg 0.00E+00 0.00E+00 0.00E+00 0.00E+00 0.00E+00 0.00E+00 0.00E+00
MR kg 0.00E+00 0.00E+00 0.00E+00 0.00E+00 2.96E+00 0.00E+00 -2.98E+00
MER kg 0.00E+00 0.00E+00 0.00E+00 0.00E+00 0.00E+00 0.00E+00 0.00E+00
EEE MJ 0.00E+00 0.00E+00 0.00E+00 0.00E+00 4.47E+01 0.00E+00 -3.13E+01
ETE MJ 0.00E+00 0.00E+00 0.00E+00 0.00E+00 3.09E+02 0.00E+00 -3.21E+02
CR Components for reuse; MR Materials for recycling; MER Materials for energy recovery; EEE Exported electric energy; ETE Exported thermal
energy
Reading example: 9,0 E-03 = 9,0*10-3 = 0,009
NEPD-2389-1125-EN NorDan NTech Villa Balcony door (security) - TE 105/80 (Without aluminium cladding)
7/9
Norwegian additional requirements
Greenhouse gas emissions from the use of electricity in the production phase
National (Poland) market with low-voltage, including production of transmission lines and grid losses, has been used for electricity in
the production process (A3).
Data source Quantity Unit
Ecoinvent v3.4 (october 2017) 1079 gram CO -ekv./kWh
2
Hazardous substances
The product contains no substances from REACH Candidate List or the Norwegian Priority List
The product contains substances below 0.1% by weight on the REACH Candidate List
The product contains substances from REACH Candidate List or the Norwegian Priority List, see table under Specific
Norwegian requirements.
The product does not contain any substances on the REACH Candidate List or the Norwegian Priority List. The product can
be characterized as hazardous waste (according to the Waste Shift, Appendix III), see table under Specific Norwegian
requirements.
Transport
Transport from production site to construction site according to scenario in A4: 1500+50 km
Indoor air quality
The product has not been tested for emissions to indoor environments.
Carbon footprint
To increase the transparency of the climate impacts, the GWP indicator has been divided into sub-indicators:
GWP-IOBC Climate impacts calculated according to instant oxidation principle
GWP-BCIP Climate impacts calculated from the net impacts of sequestration and emission of biogenic carbon
Climate impact without alu clad
Parameter Unit A1-A3 A4 A5 B1 B2 B3 B4 B5
GWP-IOBC kg CO -ekv 1.90E+02 1.28E+01 0.00E+00 0.00E+00 1.22E+01 0.00E+00 2.15E+02 0.00E+00
2
GWP-BCIP kg CO -ekv -4.88E+01 0.00E+00 6.29E+00 0.00E+00 0.00E+00 0.00E+00 -1.32E+00 0.00E+00
2
GWP kg CO -ekv 1.41E+02 1.28E+01 6.29E+00 0.00E+00 1.22E+01 0.00E+00 2.14E+02 0.00E+00
2
Climate impact without alu clad
Parameter Unit B6 B7 C1 C2 C3 C4 D
GWP-IOBC kg CO -ekv 0.00E+00 0.00E+00 0.00E+00 5.89E-01 1.11E+01 7.09E-01 -2.20E+01
2
GWP-BCIP kg CO -ekv 0.00E+00 0.00E+00 0.00E+00 0.00E+00 4.12E+01 0.00E+00 0.00E+00
2
GWP kg CO -ekv 0.00E+00 0.00E+00 0.00E+00 5.89E-01 5.23E+01 7.09E-01 -2.20E+01
2
NEPD-2389-1125-EN NorDan NTech Villa Balcony door (security) - TE 105/80 (Without aluminium cladding)
8/9
Bibliografi
NS-EN ISO 14025:2010 Miljømerker og deklarasjoner - Miljødeklarasjoner type III - Prinsipper og prosedyrer.
NS-EN ISO 14044:2006 Miljøstyring - Livsløpsvurderinger - Krav og retningslinjer
NS-EN 15804:2012+A1:2013 Bærekraftig byggverk - Miljødeklarasjoner - Grunnleggende produktkategoriregler for
byggevarer
ISO 21930:2007 Sustainability in building construction - Environmental declaration of building products
Modaresi, R. 2020 LCA-report for Nordan LCA-report nr. 325039-2 from Norwegian Institute of Wood
Technology, Oslo, Norway.
NPCR014 (04/2019) Product category rules for windows and doors, rev3, April 2019
NS-EN 16485:2014 Tømmer og skurlast - Miljødeklarasjoner - Produktkategoriregler for tre og trebaserte
produkter til bruk i byggverk
NS-EN 16449:2014 Tre og trebaserte produkter - Beregning av biogent karboninnhold i tre og omdanning til
karbondioksid
Ecoinvent v3.1-3.5 Ecoinvent database version 3.1-3.5 Centre for Life Cycle Inventories.
Statistisk sentralbyrå Tabell 04727: Fjernvarmebalansen, 2015
Statistisk sentralbyrå Tabell 09469: Nettoproduksjon av fjernvarme, 2015
NEPD-307-179-NO EPD for skurlast av gran eller furu. Treindustrien
Publisher Tlf: +47 23 08 80 00
The Norwegian EPD Foundation
Postboks 5250 Majorstuen, 0303 Oslo e-post: post@epd-norge.no
Norway web www.epd-norge.no
Owner of the declaration Tlf: +47 51 40 40 00
NorDan AS
Stasjonsveien 46, N-4460 Moi e-post: firmapost@nordan.no
Norway
web www.nordan.no
Author of the Life Cycle Assessment Tlf: +47 98 85 33 33
Roja Modaresi
Norsk Treteknisk Instiutt e-post: firmapost@treteknisk.no
Postboks 113 Blindern, 0314 Oslo, Norway web www.treteknisk.no
NEPD-2389-1125-EN NorDan NTech Villa Balcony door (security) - TE 105/80 (Without aluminium cladding)
9/9
