ver2 2015
ENVIRONMENTAL PRODUCT DECLARATION
in accordance with ISO 14025, ISO 21930 and EN 15804
Owner of the declaration: CSK Stålindustri A/S
Program operator: The Norwegian EPD Foundation
Publisher: The Norwegian EPD Foundation
Declaration number: NEPD-2694-1395-EN
Registration number: NEPD-2694-1395-EN
ECO Platform reference number: -
Issue date: 22.02.2021
Valid to: 22.02.2026
CE-Mærket stål komponenter
CE Marked steel components
CSK Stålindustri A/S
NEPD-2694-1395-EN CE-Mærket stål komponenter (ver2-april 2022)
General information
Product Owner of the declaration
CE-Mærket stål komponenter CSK Stålindustri A/S
Beams UNP-UPE-HEA-HEB-IPE-HEM Contact person: Jens Peter Frimor
Phone: +45 25 24 66 36
e-mail: jpf@csk.dk
Program operator Manufacturer
The Norwegian EPD Foundation CSK Stålindustri A/S
Post Box 5250 Majorstuen, 0303 Oslo, Norway Industrivej 7, DK-770
Phone: (+47) 23 08 80 00 Phone: +45 25 24 66 36
e-mail: post@epd-norge.no e-mail: jpf@csk.dk
Declaration number Place of production
NEPD-2694-1395-EN Denmark, Thisted
Latvia, Tukums
ECO Platform reference number Management system
EN ISO 9001
EN ISO 14001
BS/EN 1090
Product Category Rules Organisation number
EN 15804:2012 + A1:2013 serves as core PCR 20216883
NPCR 013:2019 Part B for Steel and aluminium construction
products
Statement of liability Issue date
The owner of the declaration shall be liable for the 22.02.2021
underlying information and evidence. EPD Norway shall
not be liable with respect to manufacturer information, life
cycle assessment data and evidences.
Valid to
22.02.2026
Declared unit Year of study
- 2020
Declared unit with options (A1-A4, C1-C4, D): Comparability
1kg of steel, cradle-to-gate A1-A3 with options EPD of construction products may not be comparable if they
not comply with EN 15804 and seen in a building context.
Functional unit The EPD has been worked out by
- Michael M. Jenssen, Asplan Viak AS
Verification
The CEN Norm EN 15804 serves as the core PCR.
Independent verification of the declaration and data, according
to ISO14025:2010
internal external
Approved
Third party verifier:
Ole M. K. Iversen, LCA.no AS
Independent verifier approved by EPD Norway
NEPD-2694-1395-EN CE-Mærket stål komponenter (ver2-april 2022)
2/7
Product
About CSK Steel
CSK Steel is a specialized global steel manufacturer driven by close relations with our customers. CSK Steel is certified to supply
CE marked steel structures for the European market in all Execution Classes (EXC1-EXC4).
Our quality assurance system is based on ISO 3834, and we are certified according to 1090-1. External quality audits are performed
on an ongoing basis to ensure that our certification is always valid and up-to-date.
At CSK Steel we strive to always offer - and deliver - high-quality steel structures and service, ensured by the continuous
development and improvement of our quality assurance system and policies.
We are also certified according to international standards for occupational health and safety DS/OHSAS 18001:2007 / ISO
45001:2018. Our environmental management system is certified according to ISO 14001:2015.
Product Variation
The declared product is produced by CSK in Denmark and Latvia and the results are a weighted average of the two production units;
variance is less than 10% between production sites for key environmental parameters.
Product description
CE marked steel components are structural steel beams (UNP-UPE-HEA-HEB-IPE-HEM) manufactured by CSK per customer
specification. Incoming hot-rolled profiles are first sand blasted, then cut and welded to the desired shape. Products are then surface
treated before transportation to building site.
Technical data
Dimensions: IPE 80-600, HEA/B/M 100-600, UNP/UPE 80-400, L 40-200, L 65x50 -200x150, T 30-140 and wide steels:160-500, t=5-40.
Steel grade ≤ S355. EN 10025 and EN1090-2 standards are applied.
Product specification
Materials kg %
Alloyed steel 0,93 - 0,99 93- 99
Zinc 0 - 0,06 0 - 6
Paints 0 - 0,01 0 - 1
Market
Nordics
Reference service life, product
60 years
Reference service life, building
60 years
NEPD-2694-1395-EN CE-Mærket stål komponenter (ver2-april 2022)
3/7
LCA: Calculation rules
Declared unit System boundary
1kg of steel, cradle-to-gate A1-A3 with options Modules are declared according to NPCR 013 Part B.
Declared modules are shown in Figure 1. Gray boxes denote
modules not declared.
System boundary Next system
A1 –A3 Product phase A4 C1 -C4 End-of-life D
Steel Manufacturing Transport to site Deconstruction Credits and burdens
• Sandblasting from recycling to
• Cutting avoid primary
Paint • Welding Waste transport production of steel
• Galvanization A5
and/or painting
Welding gases Wastes Installation on site Waste processing
• Steelscrap
• Wastes
Energy • Water Disposal
• VOCs and welding B1-B7
emissions
Packaging/auxiliaries Use phase
Figure 1: System boundaries
Data quality
General requirements and guidelines concerning the use of generic and specific data and the quality of those are as described in EN
15804: 2012+A1:2013, clause 6.3.6 and 6.3.7., including ISO14044:2006, 4.2.3.6. The data is representative according to temporal,
geographical and technological requirements. Database used has been ecoinvent v3.6. Calculations have been carried out using
Simapro v9. Upstream steel data from supplier EPDs:
EPD EPD programme Product type Data age
1 IBU Hot-rolled / structural section steel <10 years
2 AENOR Hot-rolled / structural section steel <10 years
3 IBU Hot-rolled / structural section steel <5 years
4 IBU Hot-rolled / structural section steel <5 years
Allocation
The allocation is made in accordance with the provisions of EN 15804. Production activities, energy, water and waste production in-
house is allocated equally among all products through mass allocation. Effects of primary production of recycled materials allocated
to the main product in which the material was used. The recycling process and transportation of the material is allocated to this
analysis.
Cut-off criteria
All major raw materials and all the essential energy is included. The production process for raw materials and energy flows that are
included with very small amounts (<1% energy, mass, impact) are not included. This cut-off rule does not apply for hazardous
materials and substances.
Benefits and loads beyond the system boundary (Module D)
Module D is calculated as net scrap * LCI for scrap, where the scrap LCI is calculated as the credit for avoided primary production of
steel, minus the burden of recycling steel scrap to make new steel, multiplied by the process yield (>1kg scrap is needed to make
1kg new steel). LCI for scrap has been provided by worldsteel (Eurofer, 2019; Worldsteel, 2017).
NEPD-2694-1395-EN CE-Mærket stål komponenter (ver2-april 2022)
4/7
LCA: Scenarios and additional technical information
The following information describe the scenarios in the different modules of the EPD.
Transport from production place to user (A4)
Type Type of vehicle Distance km Fuel/Energy Value
Capacity utilisation (incl. return) %
consumption (l/t)
Truck 44% Lorry >32t EURO5 300 0.022 l/tkm 6.6
End of Life (C1, C3, C4) Benefits and loads beyond the system (D)
Unit Value Unit Value
Hazardous waste disposed kg 0 Net new scrap kg -0.04
Collected as mixed construction waste kg 0
Reuse kg 0.00
Recycling kg 0.95
Energy recovery (C3) kg 0
To landfill (C4) kg 0.05
Transport to waste processing (C2)
Type Value
Capacity utilisation (incl. return) %
(l/t)
Waste collection 50% 19 l/tkm
Truck 26% Lorry 7,5-16t EURO5 278 0.04 l/tkm 12.2
LCA: Results
System boundaries (X=included, MND= module not declared, MNR=module not relevant)
D
lasopsiD
-gnilcyceR-yrevoceR-esueR
laitnetop
C4
X
gnissecorp
etsaW
C2
X
tropsnarT
B7 C1 C3
X X X
noitilomed
noitcurtsnoc-eD
A2
X MND MND MND
tropsnarT
esu
ygrene
lanoitarepO
Fuel/Energy
consumption
0.39 7.4
To provide a plausible scenario for transportation to waste processing, a study of Norwegian waste treatment was used as proxy
data (Raadal et al., 2009).
Use stage End of life stage
B6
MND
gnirutcafunaM
ylbmessA
esU
ecnanetniaM
riapeR
tnemecalpeR tnemhsibrufeR
esu
retaw
lanoitarepO
Type of vehicle Distance km
Beyond the
system
boundaries
tropsnarT
End of life scenario
Net new scrap is calculated by substracting the scrap content of outgoing steel from the recycling rate. The weighted average
scrap content is 99% from suppliers. Note that outgoing scrap and the parameter for Secondary Material content (SM) differ,
wherein the latter accounts for the total amount of scrap needed in the system to fulfill the declared unit.
A 95% recovery rate is assumed, wherein 5% is assumed landfilled - in effect providing a 95% recycling rate. Reuse is not
included in this scenario.
Lorry 21t
Product stage Assemby stage
A1 A3 A4 B1 B2 B5
X X X MND MND MND
slairetam
waR
Scenario for distance to building site according to NPCR 013 Part B.
A5 B3 B4
MND
NEPD-2694-1395-EN CE-Mærket stål komponenter (ver2-april 2022)
5/7
Environmental impact
Parameter Unit A1-A3 A4 C1 C2 C3 C4 D
GWP kg CO -eqv 1.16E+00 2.59E-02 2.15E-02 6.86E-02 2.19E-04 5.30E-05 6.86E-02
2
ODP kg CFC11-eqv 4.13E-08 5.11E-09 3.87E-09 1.23E-08 2.61E-11 1.77E-11 -3.84E-10
POCP kg C 2H 4 -eqv 3.93E-04 4.13E-06 4.30E-06 1.14E-05 5.97E-08 1.94E-08 2.98E-05
AP kg SO 2 -eqv 5.53E-03 8.37E-05 1.63E-04 2.47E-04 1.25E-06 3.95E-07 1.36E-04
EP kg PO 43--eqv 7.50E-04 1.42E-05 3.51E-05 4.63E-05 2.73E-07 6.81E-08 1.49E-05
ADPM kg Sb-eqv 2.74E-05 5.06E-08 7.21E-09 1.54E-07 2.15E-09 6.10E-11 2.17E-07
ADPE MJ 1.45E+01 4.08E-01 3.09E-01 9.89E-01 2.91E-03 1.51E-03 9.98E-01
GWP Global warming potential; ODP Depletion potential of the stratospheric ozone layer; POCP Formation potential of tropospheric
photochemical oxidants; AP Acidification potential of land and water; EP Eutrophication potential; ADPM Abiotic depletion potential for non
fossil resources; ADPE Abiotic depletion potential for fossil resources
Resource use
Parameter Unit A1-A3 A4 C1 C2 C3 C4 D
RPEE MJ 1.35E+00 6.51E-03 1.66E-03 1.02E-02 1.51E-02 2.80E-05 4.43E-02
RPEM MJ 1.45E+00 0.00E+00 0.00E+00 0.00E+00 0.00E+00 0.00E+00 0.00E+00
TPE MJ 2.80E+00 6.51E-03 1.66E-03 1.02E-02 1.51E-02 2.80E-05 4.43E-02
NRPE MJ 1.06E+01 4.20E-01 3.12E-01 1.01E+00 3.78E-03 1.54E-03 1.02E+00
NRPM MJ 5.60E+00 0.00E+00 0.00E+00 0.00E+00 0.00E+00 0.00E+00 0.00E+00
TRPE MJ 1.62E+01 4.20E-01 3.12E-01 1.01E+00 3.78E-03 1.54E-03 1.02E+00
SM kg 1.15E+00 0.00E+00 0.00E+00 0.00E+00 0.00E+00 0.00E+00 0.00E+00
RSF MJ 0.00E+00 0.00E+00 0.00E+00 0.00E+00 0.00E+00 0.00E+00 0.00E+00
NRSF MJ 5.14E-03 0.00E+00 0.00E+00 0.00E+00 0.00E+00 0.00E+00 6.24E-02
W m3 3.84E-03 8.91E-05 4.22E-05 4.22E-05 4.22E-05 1.69E-06 4.50E-08
RPEE Renewable primary energy resources used as energy carrier; RPEM Renewable primary energy resources used as raw materials; TPE
Total use of renewable primary energy resources; NRPE Non renewable primary energy resources used as energy carrier; NRPM Non
renewable primary energy resources used as materials; TRPE Total use of non renewable primary energy resources; SM Use of secondary
materials; RSF Use of renewable secondary fuels; NRSF Use of non renewable secondary fuels; W Use of net fresh water
End of life - Waste
Parameter Unit A1-A3 A4 C1 C2 C3 C4 D
HW kg 8.37E-02 2.13E-07 1.39E-07 5.10E-07 5.54E-09 1.08E-09 -1.75E-17
NHW kg 2.73E-02 3.66E-02 3.40E-04 3.46E-02 1.05E-04 1.00E-02 0.00E+00
RW kg 2.52E-04 2.95E-06 2.17E-06 7.01E-06 2.12E-08 9.96E-09 0.00E+00
HW Hazardous waste disposed; NHW Non hazardous waste disposed; RW Radioactive waste disposed
End of life - Output flow
Parameter Unit A1-A3 A4 C1 C2 C3 C4 D
CR kg 3.40E-02 0.00E+00 0.00E+00 0.00E+00 0.00E+00 0.00E+00 0.00E+00
MR kg 0.00E+00 0.00E+00 0.00E+00 0.00E+00 9.50E-01 0.00E+00 0.00E+00
MER kg 0.00E+00 0.00E+00 0.00E+00 0.00E+00 0.00E+00 0.00E+00 0.00E+00
EEE MJ 0.00E+00 0.00E+00 0.00E+00 0.00E+00 0.00E+00 0.00E+00 0.00E+00
ETE MJ 0.00E+00 0.00E+00 0.00E+00 0.00E+00 0.00E+00 0.00E+00 0.00E+00
CR Components for reuse; MR Materials for recycling; MER Materials for energy recovery; EEE Exported electric energy; ETE Exported thermal
energy
Reading example: 9,0 E-03 = 9,0*10-3 = 0,009
NEPD-2694-1395-EN CE-Mærket stål komponenter (ver2-april 2022)
6/7
Additional Norwegian requirements
Greenhous gas emission from the use of electricity in the manufacturing phase
Norwegian production mix from import, medium voltage (production of transmission lines, in addition to direct emissions and losses
in grid) of applied electricity for the manufacturing prosess (A3).
Data source Amount Unit
Econinvent v3.6 - Denmark 0.359 kg CO -eqv/kWh
2
Econinvent v3.6 - Latvia 0.604 kg CO -eqv/kWh
2
Dangerous substances
The product contains no substances given by the REACH Candidate list or the Norwegian priority list
The product contains substances given by the REACH Candidate list or the Norwegian priority list that are less than 0,1 % by
weight.
The product contain dangerous substances, more then 0,1% by weight, given by the REACH Candidate List or the
Norwegian Priority list, see table.
The product contains no substances given by the REACH Candidate list or the Norwegian priority list. The product is classified
as hazardous waste (Avfallsforskiften, Annex III), see table.
Indoor environment
No tests have been carried out on the product concerning indoor climate - Not relevant.
Carbon footprint
Carbon footprint has not been worked out for the product.
Bibliography
ISO 14025:2010 Environmental labels and declarations - Type III environmental declarations - Principles and
procedures
ISO 14044:2006 Environmental management - Life cycle assessment - Requirements and guidelines
EN 15804:2012+A1:2013 Sustainability of construction works - Environmental product declaration - Core rules for the
product category of construction products
ISO 21930:2007 Sustainability in building construction - Environmental declaration of building products
Jennssen, M.M. (2020) LCA report for CSK Stålindustri A/S
NPCR 013:2019 Part B for Steel and Aluminium products
Raadal et al. (2009) Klimaregnskap for avfallshåndtering. Fase I og II: Glassemballasje, metallemballasje, papir,
papp, plastemballasje, våtorganisk avfall, treavfall og restavfall fra husholdninger. ISBN: 82-
8035-073-X.
Publisher/Program operator Phone: +47 23 08 80 00
The Norwegian EPD Foundation
Post Box 5250 Majorstuen, 0303 Oslo e-mail: post@epd-norge.no
Norway web epd-norge.no
Owner of the declaration Phone: +45 25 24 66 36
CSK Stålindustri A/S Fax
Industrivej 7, DK-770 e-mail: jpf@csk.dk
Denmark web csk.dk
Author of the Life Cycle Assessment Phone: +47 41 79 94 17
Michael M. Jenssen Fax
Asplan Viak AS e-mail: asplanviak@aplanviak.no
Abels gate 9, 7030 Trondheim, Norway web asplanviak.no
NEPD-2694-1395-EN CE-Mærket stål komponenter (ver2-april 2022)
7/7
