1114 NEPD
Ver. 2 2015(17)
ENVIRONMENTAL PRODUCT DECLARATION
in accordance with ISO 14025, ISO 21930 and EN 15804
Owner of the declaration: Flügger Norway AS
Program operator: The Norwegian EPD Foundation
Publisher: The Norwegian EPD Foundation
Declaration number: NEPD-1995-881-EN
Registration number: NEPD-1995-881-EN
ECO Platform reference number: -
Issue date: 07.01.2020
Valid to: 07.01.2025
Flutex 5S™
Flügger Norway AS
www.epd-norge.no
General information
Product: Owner of the declaration:
Flutex 5S™ Flügger Norway AS
contact person: Stine Rosendal Tangaa
phone: +45 40 64 75 98
e-mail: regulatoryaffairs@flugger.com
Program operator: Manufacturer:
The Norwegian EPD Foundation Flügger Denmark A/S
Pb. 5250 Majorstuen, 0303 Oslo
Tlf: +47 23 08 82 92
e-post: post@epd-norge.no
Declaration number: Place of production:
NEPD-1995-881-EN Vejlevej 150, 6000 Kolding, Denmark
ECO Platform reference number: Management system:
ISO 14001:2015 (DK011198)
ISO 9001:2015 (DK007923)
This declaration is based on PCR: Org. no.:
NS-EN 15804:2012+A1:2013 serves as core PCR. 928 380 173
Product descriptions based on "IBU PCR Part B for coatings
with organic binders". This also applies to products with
inorganic binders.
Issue date:
Statement of liability: 07.01.2020
The owner of the declaration shall be liable for the underlying
informationandevidence.EPDNorwayshallnotbeliablewith
respect to manufacturer information, life cycle assessment
data and evidences. Valid to:
07.01.2025
Declared unit: Year of study:
1 kg Flutex 5S paint delivered to market 2019
Declared unit with option: Comparability:
EPD of construction products may not be comparable if they
do not comply with NS-EN 15804 and seen in a building
context.
Functional unit: Author of the Life Cycle Assessment:
Mafalda Silva
Østfoldforskning AS
Verification:
Independent verification of data, other environmental
information and the declaration according to ISO14025:2010, §
8.1.3 and § 8.1.4
internal external
Approved
Third party verifier:
PhD Ellen Soldal, Researcher
(Independent verifier approved by EPD Norway)
NEPD-1995-881-EN Flutex-5S™_ENG 2/9
Product
Product description: Technical data:
Flutex 5S is a water based, rich PVA-paint. It gives a matte Density: 1,44 kg/l:
and uniform structure, with subdued gloss. The white variants Solids by volume: 56,0%
and Base 1 are ecolabelled with EU Ecolabel. The entire EU VOC limit value for product (Cat. A/a): 30 g/l
Flutex 5S series is registered in the Nordic Ecolabelling Product VOC max. 10 g/l
Building Products Database.
Nominal spreading rate: 8 - 9 m2/l
Flutex 5S is recommended for wall and ceilings with normal Wet film thickness: 113 - 125 µm
functional requirements, that are exposed to moderate dirt, Dry film thickness: 40 - 44 µm
wear and tear. Withstands cleaning with water and wiping with
a damp cloth. The most representative and worst case formulation is chosen
forthisEPD.Forproductswithaselectionofcolours,thiswill
For information on Green Building Standard credits and be the formulation with the highest content of titanium dioxide.
Ecolabels, see "Additional Information" on page 4.
The product packaging is based on an average sized plastic
Product specification:
packaging.
Life cycle analysis carried out for the white variant, which is
estimated to have the greatest environmental impact.
For safety, health and environmental conditions, see the
Safety Data Sheet for the declared product on
The material composition of the declared product:
www.flugger.no.
Materials %
Water 30-35
For information on technical data, application and use of the
Binder 30-35
product,seetheTechnicalDataSheetandFDV(Forvaltning,
Extender 25-30
Drift og Vedlikehold) for the declared product on
Titanium dioxide 15-20
www.flugger.no
Solvent < 1
Additive < 2
Biocide < 0,5 Market:
Scandinavia and Europe
Packaging kg
Wooden packaging - pallet 0 Reference service life, product
Plastic packaging - pallet # The reference service life of the product is highly dependent
Plastic packaging # on the conditions of use.
Estimated service life, object
The coated object is not declared.
LCA: Calculation rules
Declared unit: System boundary:
1 kg Flutex 5S paint delivered to market The flow chart below illustrates the system boundaries for the
analysisaccordingtothemoduleprincipleinNS-EN15804.The
analysis is carried out from cradle-to-gate (A1-A3), including
module A4 transport to market.
A1 A2 A3 A4 A5 B1-B7 C1-C4 D
Raw materials Transport Production Transport to Application and Usephase Endof life Benefits of
market installation recovery
Preassemblyof
raw materials
Rawmaterial Transport of
extraction and raw materials
production Dispersionof
pigments
Transportof Module not Module not Module not Module not
product to declared declared declared declared
market
Mixing
Packaging Transport of
production packaging
QCcheck and
adjustment
Fillingand
labelling
Systemboundaries«Cradle-to-gate»
System boundary for this EPD
NEPD-1995-881-EN Flutex-5S™_ENG 3/9
System boundary for this EPD
Data quality:
The CEPE database is used as basis for the raw material composition. Specific datafor theproduct composition and rawmaterial
amounts has been provided bythe manufacturer and represents the production of the declared product. Production site data was
collectedin2018.RemainingdataisbasedonEcoinventv3.5,butadjustedtoimproverepresentativeness.Allenergyconsumption
in the database is assumed not to be used as raw material.
Cut-off criteria: Allocation:
All major raw materials and essential energy is included. The Theallocationismadeinaccordancewiththeprovisionsof
production process for raw materials and energy flows with very EN15804.Incomingenergy,waterandwasteproductionin-
smallamounts(<1%)arenotincluded.Thesecut-offcriteriadonot house is primarily allocated equally among all products
apply for hazardous materials and substances. through mass allocation. The recycling process and
transportation of the material is allocated to this analysis.
Additional information:
The declared product contributes to Green Building Standard credits by meeting the following specific requirements:
-Emmision criteria according to M1 (<0,2mg/m2/h after 28 days)
-EU Ecolabel (SE/044/002)
-Properties criteria in BASTA (2019:A1)
-Accepted according to Byggvarubedömningens Assessment Criteria 5.0 (2019)
-Class B according to SundaHus Material Data Assessment Criteria 6.1.5 (2019)
BREEAM®NOR (2016)
HEA 02: VOC content for "Interior matt walls and ceilings" (30 g/l) (EU Directive 2004/42/CE) and emission criteria (ISO 16000-series).
Mat01:TheproductcontainsnosubstancesontheNorwegianTechnicalCheckList(A20),whichexceedsthelimitvalueforhealthand
environment.
BREEAM®NOR (2012)
HEA 9: VOC content for "Interior matt walls and ceilings" (30 g/l) (EU Directive 2004/42/CE) and emission criteria (ISO 16000-series).
Mat1.5:TheproductcontainsnosubstancesontheNorwegianTechnicalCheckList(A20),whichexceedsthelimitvalueforhealthand
environment.
Additional certificates and approvals may be available on request.
NEPD-1995-881-EN Flutex-5S™_ENG 4/9
LCA: Scenarios and additional technical information
The following information describe the scenarios in the different modules of the EPD.
The only declared module after the factory gate is A4 transport to market.
Transport from production place to user (A4)
Capacity utilisation (incl. Fuel/Energy
Type Type of vehicle Distance km Unit
return) % consumption
Truck, Europe,
Truck 53.00 % 573 0.0192 kg/tkm
EURO 6
Railway
Boat
Other
Construction/Installation (A5) Use (B1)
Unit Value Unit Value
Auxiliary kg Relevant emissions during use kg
Water consumption m3
Electricity consumption kWh
Other energy carriers MJ
Material loss kg
Dust in the air kg
VOC emissions kg
Maintenance (B2)/Repair (B3) Replacement (B4)/Refurbishment (B5)
Unit Value Unit Value
Maintenance cycle* Replacement cycle* stk
Auxiliary kg Electricity consumption kWh
Other resources kg Replacement of worn parts 0
Water consumption m3 * Value or refence shelf-life
Electricity consumption kWh
Other energy carriers MJ
Material loss kg
VOC emissions kg
Operational energy (B6) and water consumption (B7) End of life (C1, C3, C4)
Unit Value Unit Value
Water consumption m3 Hazardous waste disposed kg
Electricity consumption kWh Collected as mixed construction waste kg
Other energy carriers MJ Reuse kg
Power output of equipment kW Recycling kg
Energy recovery kg
Til landfill kg
Transport to waste processing (C2)
Capacity utilisation (incl. Fuel/Energy
Type Type of vehicle Distance km Unit Value (l/t)
return) % consumption
Truck
Railway
Boat
Other
NEPD-1995-881-EN Flutex-5S™_ENG 5/9
LCA: Results
System boundaries (X=included, MND=module not declared, MNR=module not relevant)
MND MND
Environmental impact
POCP kg CH -eq. 2 4
kg SO -eq. 2
kg PO 43--eq. 1.12E-05
kg Sb -eq. 8.86E-06 7.54E-06
MJ 2.49E+01 1.21E+00
GWP Global warming potential; ODP Depletion potential of the stratospheric ozone layer; POCP Formation potential of tropospheric
photochemical oxidants; AP Acidification potential of land and water; EP Eutrophication potential; ADPM Abiotic depletion potential for non fossil
resources; ADPE Abiotic depletion potential for fossil resources
tnemecalpeR
B7
tnemhsibrufeR gnissecorp
etsaW
MND
7.74E-06
AP 1.31E-04
EP 1.23E-03 1.78E-05
9.65E-08
3.18E-01 8.10E-01
tropsnarT
7.33E-04 3.44E-06
9.62E-03 6.88E-05 1.01E-03
5.70E-08
tropsnarT tropsnarT
/noitcurtsnoC egats
noitallatsni esU
ecnanetniaM
esu
ygrene
lanoitarepO
esu
retaw
lanoitarepO
Construction/
installation stage
riapeR
User stage
slairetam
waR
Beyond the
Product stage End of life stage system
boundaries
A4 B5 C1
X X MND MND
7.92E-09
5.00E-05
2.47E-04
gnirutcafunaM
A3 C2
noitilomed
/noitcurtsnoceD
A2 B1 B2 B4 B6
MND MND
1.50E-07
-gnilcycer/yrevocer/esueR
laitnetop
C4 D
X X MND
Parameter A2 A4
2.07E-02 4.93E-02
3.87E-09 9.90E-09
ADPM
ADPE
lasopsid
etsaW
A1 A5 B3 C3
MND MND MND MND MND
Unit A1 A3
GWP kg CO 2 -eq. 1.53E+00 1.45E-01
ODP kg CFC11-eq.
NEPD-1995-881-EN Flutex-5S™_ENG 6/9
Resource use
Parameter Unit A1 A2 A3 A4
RPEE MJ 8.05E-01 3.55E-03 5.84E-01 8.73E-03
RPEM MJ 0.00E+00 0.00E+00 1.74E-02 0.00E+00
TPE MJ 8.05E-01 3.55E-03 6.01E-01 8.73E-03
NRPE MJ 1.36E+01 3.23E-01 1.55E+00 8.24E-01
NRPM MJ 1.39E+01 0.00E+00 0.00E+00 0.00E+00
TRPE MJ 2.75E+01 3.23E-01 1.55E+00 8.24E-01
SM kg 0.00E+00 0.00E+00 0.00E+00 0.00E+00
RSF MJ 0.00E+00 0.00E+00 0.00E+00 0.00E+00
NRSF MJ 0.00E+00 0.00E+00 0.00E+00 0.00E+00
W m3 4.77E-01 6.16E-05 1.16E-03 1.77E-04
RPEERenewableprimaryenergyresourcesusedasenergycarrier;RPEMRenewableprimaryenergyresourcesusedasrawmaterials;TPE
Total use of renewable primary energy resources; NRPE Non renewable primary energy resources used as energy carrier; NRPM Non
renewable primary energy resources used as materials; TRPE Total use of non renewable primary energyresources; SM Use of secondary
materials; RSF Use of renewable secondary fuels; NRSF Use of non renewable secondary fuels; W Use of net fresh water
End of life - Waste
Parameter Unit A1 A2 A3 A4
HW kg 2.10E-05 2.04E-07 5.44E-06 4.77E-07
NHW kg 3.78E-01 2.21E-02 1.58E-01 7.43E-02
RW kg 2.16E-04 2.18E-06 6.48E-06 5.60E-06
HW Hazardous waste disposed; NHW Non hazardous waste disposed; RW Radioactive waste disposed
End of life - Output flow
Parameter Unit A1 A2 A3 A4
CR kg 0.00E+00 0.00E+00 0.00E+00 0.00E+00
MR kg 0.00E+00 0.00E+00 5.55E-03 0.00E+00
MER kg 0.00E+00 0.00E+00 3.20E-05 0.00E+00
EEE MJ 0.00E+00 0.00E+00 1.69E-03 0.00E+00
ETE MJ 0.00E+00 0.00E+00 1.79E-02 0.00E+00
CR Components for reuse; MR Materials for recycling; MER Materials for energy recovery; EEE Exported electric energy; ETE Exported thermal
energy
Reading example: 9,0 E-03 = 9,0*10-3 = 0,009
NEPD-1995-881-EN Flutex-5S™_ENG 7/9
Additional requirements
Greenhouse gas emissions from the use of electricity in the manufacturing phase
Nationalproductionmixfromimport,lowvoltage(productionoftransmissionlines,inadditiontodirectemissionsandlossesingrid)
of applied electricity for the manufacturing process (A3). Background data is presented inthe tablebelow. Characterisationfactors
from NS-EN 15804:2012+A1:2013 are used.
Electricity mix Data source Value Unit
Electricity, Denmark (kWh) ecoinvent 3.5 367 g CO -eq./kWh
2
Dangerous substances
The product contains no substances given by the REACH Candidate list or the Norwegian priority list
The product contains substances given by the REACH Candidate list <0,1 weight%
The product contains substances given by the REACH Candidate list or the Norwegian priority list, see table above
The product contains no substances given by the REACH Candidate list or the Norwegian priority list. The product is
chracaterised as hazardous waste (acc. to the Waste Directive, Appendix III), se table above.
Indoor environment
The declared product is emission tested according to the ISO-16000 series (2006).
NEPD-1995-881-EN Flutex-5S™_ENG 8/9
Bibliography
BASTA (2018) Properties criteria - BASTA, version 2019:A1
BREEAM®NOR (2012) BREEAM-NOR for new contructions 2012, SD 5066A, version 1.1. The Norwegian Green Building
Council
BREEAM®NOR (2016) BREEAM-NOR for new contructions 2016, SD 5075NOR, version 1.1. The Norwegian Green Building
Council
Byggvarubedömningen (2019) Assessment criteria for chemical content and lifecycle aspects, version 5.0
SundaHus (2019) Material Data Assessment Criteria, version 6.1.5
EU Ecolabel SE/044/002 - Flügger Flutex 5S Vit
Building Information Foundation (2017) M1 Emission Classification of Building Materials: Protocol for Chemical and Sensory Testing of
Building Materials”, v. 15.11.2017
CEPE v3.0 Raw materials LCI database for the European coatings and printing ink industries
Ecoinvent v3.5 Alloc Rec, Swiss Centre of Life Cycle Inventories. www.ecoinvent.ch
NS-EN ISO 14025:2010 Environmental labels and declarations - Type III environmental declarations - Principles and
procedures
NS-EN ISO 14044:2006 Environmental management - Life cycle assessment - Requirements and guidelines
NS-EN 15804:2012+A1:2013 Environmental product declaration - Core rules for the product category of construction products
NS-EN PCR Part A Construction Products and Services. Version 1.0. EPD Norge
IBU PCR Part B Requirements on the EPD for Coatings with organic binders. v1.7, January 2019
ISO 16000-series Indoor air standards for VOCs sampling and determination, i.e. 9 (2006)
EN 15251 (2007) Indoor environmental input parameters for design and assessment of energy performance of
buildings addressing indoor air quality, thermal environment, lighting and acoustics. CEN, Brussels
EU Directive 2004/42/CE The limitation of emissions of volatile organic compounds due to the use of organic solvents in certain
paints and varnishes and vehicle refinishing products
REACH Candidate List (2018) Candidate List of substances of very high concern for Authorisation IAW Article 59(10) of the REACH
Regulation
Technical Check List (A20) and Miljøgiftlisten, The Norwegian Environment Agency
Norwegian Priority List (2018)
Dahlgren,L., Jelse,K., Skenhall,S.A., Ljungkvist,H., Westerdahl,J., Stripple,H., Högberg,J. and Rydberg,T. (2014). Raw materials LCI database
for the European coatings and printing ink industries-Documentation of datasets v.2.0, IVLU4859, August 2014
Dahlgren,L., Stripple,H., Oliveira,F., Rydberg,T., and Zhang,Y. (2016). Raw materials LCI database for the European coatings and printing ink
industries - Documentation of data sets v. 3.0, IVL U5659, May 2016.
Program operator and publisher phone: +47 977 22 020
The Norwegain EPD Foundation
Post Box 5250 Majorstuen, 0303 Oslo e-mail: post@epd-norge.no
Norway web www.epd-norge.no
Owner of the declaration phone: +47 23 30 21 90
Flügger Norway AS
Karoline Kristiansens vej 4 e-mail: regulatoryaffairs@flugger.com
0661 Oslo, Norway web www.flugger.com
Author of the Life Cycle Assesment phone: +47 69 35 11 00
Mafalda Silva fax: +47 69 34 24 94
Østfoldforskning AS e-mail: post@ostfoldforskning.no
Stadion 4, 1671 Kråkerøy, Norge web www.ostfoldforskning.no
NEPD-1995-881-EN Flutex-5S™_ENG 9/9
