Ver. 1 2015
environmental product declaration
in accordance with ISO 14025
Owner of the declaration: Cav. Uff. Giacomo Cimberio S.p.A.
Program operator: The Norwegian EPD Foundation
Publisher: The Norwegian EPD Foundation
Declaration number: NEPD-2147-970-EN
Registration number: NEPD-2147-970-EN
ECO Platform reference number: -
Issue date: 29.04.2020
Valid to: 29.04.2025
Product-specific Type III EPD of Cimberio valves
Cav. Uff. Giacomo Cimberio S.p.A.
www.epd-norge.no
NEPD-2147-970-EN Product-specific Type III EPD of Cimberio valves (ver2-200421)
General information
product owner of the declaration
1 kg of valves for system plants of different sectors Cav. Uff. Giacomo Cimberio S.p.A. - VAT nr: IT 00122640030
Contact person: Roberto Cimberio
Phone: +39 0322 923001
e-mail: info@cimberio.it
Address: Via Torchio, 57- C.P. 106 - 28017 San Maurizio
d’Opaglio (NO) - Italy
program holder manufacturer
The Norwegian EPD Foundation Cav. Uff. Giacomo Cimberio S.p.A.
Postboks 5250 Majorstuen, 0303 Oslo Via Torchio, 57- C.P. 106 - 28017, San Maurizio d’Opaglio
Phone: +47 23088292 (NO) - Italy
e-mail: post@epd-norge.no Phone: +39 0322 923001
e-mail: info@cimberio.it
declaration number place of production
NEPD-2147-970-EN Via Torchio, 57- C.P. 106 - 28017, San Maurizio d’Opaglio
(NO) - Italy
eco platform reference number management system
- ISO 9001, ISO 14001, ISO 45001, ISO 50001, PAS 99,
SA 8000
this declaration is based on product category rules:
CEN Standard EN 15804:2012+a2:2019 serves as core PCR
organization no:
“Products and Services - Part B: Requirements on the EPD for
Bathroom fittings and showers” of Institut Bauen und Umwelt VAT nr: IT 00122640030
e.V. (IBU)
Statements issue date
The owner of the declaration shall be liable for the underlying 29.04.2020
information and evidence.
EPD Norway shall not be liable with respect to manufacturer,
life cycle assessment data and evidences. valid to
29.04.2025
declared unit Year of study
1 kg of valves (motorized valves excluded) 2018
declared unit with option comparability
- EPD of construction products may not be comparable if they
not comply with EN 15804 and seen in a plants context.
Functional unit the epd has been worked out by
1 kg of valves (motorized valves excluded) Arch. Ph.D. Ganassali Sara (A2life)
Verification
Independent verification of the declaration and data, Approved
according to ISO14025:2010
internal X external
Third party verifier:
Ing. Vito D’Incognito – Take Care International
(Independent verifier approved by EPD Norway)
NEPD-2147-970-EN Product-specific Type III EPD of Cimberio valves (ver2-200421) 2/8
product
product description technical data
Different types of valves for system plants of different sectors. valves tested according to EN 12266-1 standard. Brass alloys
The process starts with the manufacturing of raw brass and used for valves complie with standard EN 12165. Brass alloys
bronze pieces for valves obtained from casting and hot-moulding contains low percentage of lead (less than admitted by DM
(activities carried out by external subcontractors); then the pieces 174/2004).
are mechanically worked and assembled with valves components
(e.g. handles, gaskets, balls, fittings, etc.). Some pieces and valve
components are coated with chrome and powder, according to market
the valve typologies in which they are used. Italy, Norway, rest of World (mainly where manufacturer’s
Declared unit refer to different numbers and types of valves; branches are located)
every valve typology contains valves with different dimensions
and weights. However, the same manufacturing process and the
similarities of valves allow a declared unit based on mass unit of reference service life
products. average reference service life (RSL) of 12 years. The average
Motorized valves are excluded from this EPD. RSL is the average value between valves warranty (5 years)
Product specification
Product specification per 1 kg of valves is given below.
Materials kg %
Brass 0,895 89,5
Aluminium 0,0450 4,50
Steel 0,0192 1,92
PTFE 0,00748 0,75
Bronze 0,00580 0,58
PA 0,00269 0,27
EPDM and NBR 0,00246 0,25
Other materials 0,0223 2,23
NEPD-2147-970-EN Product-specific Type III EPD of Cimberio valves (ver2-200421) 3/8
lca: calculation rules
declared unit technical data
1 kg of valves (motorized valves excluded) Cradle-to-gate system boundaries with transportation towards
manufacturer’s Norwegian warehouse. All processes from raw
materials extraction (module A1) to transports (module A2) and
production at the manufacturing site (module A3) are included
in the analysis (Product stage, modules A1-3). Transport
towards Norway is illustrated in module A4.
a1 a2 a3 a4
Brass Transport Subcontractors Subcontractors
Raw material (casting - moulding) (chrome and powder
coating, sandblasting,
assembly)
Bronze raw pieces and Transport
valve components
Packaging and Transport Transport
ancillary products
Manufacturing
in plant
Energy from the grid
Heat from natural gas
Energy from
Water
PV panels
data quality allocation
General requirements and guidelines concerning use of generic The allocation is made in accordance with the provisions of
and specific data and the quality of those are as described in EN EN 15804. Incoming energy and water and waste production
15804:2012 + A2:2019, clause 6.3.8. The data is representative in-house is allocated equally among all products through mass
according to temporal, geographical and technological allocation. Effects of primary production of recycled materials
requirements. allocated to the main product in which the material was used
(the recycling process and transportation of the material is not
Temporal: data used in module A3 is provided by the manufacturer considered in this analysis with cradle-to-gate boundaries).
and refers to 2018 total use of materials and energy consumption
for production of 1 kg of valves. Generic data and data gaps
have been created and/or taken from Ecoinvent 3.6 in SimaPro
Cut-off criteria
software.
All major raw materials and all the essential energy is included.
The production process for raw materials and energy flows that
Geographical: the geographic region of the production sites for
are included with very small amounts (<1%) are not included.
raw materials included in the calculation is Europe and rest of
This cut-off rule does not apply for hazardous materials and
World (according to specific raw material); the geographic region
substances.
of energy and water consumption used in manufacturing site is
Europe and Italy.
Technological: data represents technology in use.
NEPD-2147-970-EN Product-specific Type III EPD of Cimberio valves (ver2-200421) 4/8
lca: results
System boundaries (X=included, MND=module not declared, MNR=module not relevant)
Beyond the
Product stage Assembly stage Use stage End of life stage system
boundaries
slairetam
waR
tropsnarT
gnirutcafunaM
tropsnarT ylbmessA
esU
ecnanetniaM
riapeR
tnemecalpeR
tnemhsibrufeR
esu
ygrene
lanoitarepO
esu
retaw
lanoitarepO
noitcurtsnoc-eD
noitilomed tropsnarT
gnissecorp
etsaW
lasopsiD
-yrevoceR-esueR
laitnetop-gnilcyceR
lca: Scenarios and additional technical information
The following information describe the scenarios in the different modules of the EPD.
Transportation toward Norwegian manufacturer’s branch warehouse is described in the following Table.
transport from production place to user (a4)
Type Capacity utilisation Type of vehicle Distance km Fuel/Energy Value
(incl. return) % consumption (l/t)
Truck 92,5% Lorry Truck 24 ton 2250 0,015 l/tkm 0,357 l/km
The environmental impacts generated in the life cycle stages assessed within the system boundaries are calculated using the Simapro
Software, version 9.0.0.49. Background data is from Simapro database (Ecoinvent 3.6). The impact assessment methodologies used
are CML-IA Baseline (according to EN 15804:2012), EDIP 2003, Cumulative Energy Demand and AWARE (for water depletion).
A1 A2 A3 A4 A5 B1 B2 B3 B4 B5 B6 B7 C1 C2 C3 C4 D
X X X X MND MND MND MND MND MND MND MND MND MND MND MND MND
Environmental Impacts
parameter unit a1 a2 a3 a1-3 a4
GWP kg CO-eqv 6,39E+00 1,55E-02 7,64E-01 7,17E+00 3,65E-01
2
ODP kg CFC11-eqv 3,26E-05 3,01E-09 1,03E-07 3,27E-05 6,72E-08
POCP kg CH-eqv 7,75E-03 2,52E-06 2,89E-04 8,04E-03 5,45E-05
2 4
AP kg SO-eqv 1,91E-01 5,46E-05 6,86E-03 1,98E-01 8,61E-04
2
EP kg PO3--eqv 1,24E-01 1,26E-05 1,26E-03 1,26E-01 1,93E-04
4
ADPM kg Sb-eqv 2,94E-03 2,79E-08 2,83E-06 2,94E-03 1,04E-06
ADPE MJ 6,95E+01 2,46E-01 9,66E+00 7,94E+01 5,50E+00
GWP Global warming potential; ODP Depletion potential of the stratospheric ozone layer; POCP Formation potential of tropospheric
photochemical oxidants; AP Acidification potential of land and water; EP Eutrophication potential; ADPM Abiotic depletion potential for
non fossil resources; ADPE Abiotic depletion potential for fossil resources
NEPD-2147-970-EN Product-specific Type III EPD of Cimberio valves (ver2-200421) 5/8
Resource use
parameter unit a1 a2 a3 a1-3 a4
RPEE MJ 1,20E+01 2,72E-03 3,23E+00 1,52E+01 6,21E-02
RPEM MJ - - - - -
TPE MJ 1,20E+01 2,72E-03 3,23E+00 1,52E+01 6,21E-02
NRPE MJ 9,67E+01 2,66E-01 1,23E+01 1,09E+02 5,94E+00
NRPM MJ - - - - -
TRPE MJ 9,67E+01 2,66E-01 1,23E+01 1,09E+02 5,94E+00
SM kg 6,76E-01 - - 6,76E-01 -
RSF MJ - - - - -
NRSF MJ - - - - -
W m3 2,97E+00 1,47E-03 4,62E-01 3,43E+00 2,91E02
RPEE Renewable primary energy resources used as energy carrier; RPEM Renewable primary energy resources used as raw materials;
TPE Total use of renewable primary energy resources; NRPE Non renewable primary energy resources used as energy carrier; NRPM
Non renewable primary energy resources used as materials; TRPE Total use of non renewable primary energy resources; SM Use of
secondary materials; RSF Use of renewable secondary fuels; NRSF Use of non renewable secondary fuels; W Use of net fresh water
End of life - Waste
parameter unit a1 a2 a3 a1-3 a4
HW kg 1,15E-03 1,37E-07 1,09E-02 1,21E-02 3,29E-06
NHW kg 1,26E+00 2,12E-02 1,10E-01 1,39E+00 2,68E-01
RW kg 2,67E-04 1,70E-06 3,70E-05 3,06E-04 3,79E-05
HW Hazardous waste disposed; NHW Non hazardous waste disposed; RW Radioactive waste disposed
End of life - Output flows
parameter unit a1 a2 a3 a1-3 a4
CR kg - - - - -
MR kg 3,76E-02 - 5,44E-01 5,82E-01 -
MER kg - - - - -
EEE MJ - - 5,58E-02 5,58E-02 --
ETE MJ - - - - -
CR Components for reuse; MR Materials for recycling; MER Materials for energy recovery; EEE Exported electric energy; ETE Exported
thermal energy
Reading example: 9,0 E-03 = 9,0*10-3 = 0,009
NEPD-2147-970-EN Product-specific Type III EPD of Cimberio valves (ver2-200421) 6/8
additional norwegian requirements
Greenhous gas emission from the use of electricity in the manufacturing phase
National production mix from import, low woltage (production of transmission lines, in addition to direct emissions and losses in grid)
of applied electricity for the manufacturing prosess (A3).
Data source Amount Unit
Ecoinvent 3.6 (April 2020) 0,364 kgCO-eqv/kWh
2
dangerous substances
The product contains no substances given by the REACH Candidate list or the Norwegian priority list
The product contains substances given by the REACH Candidate list or the Norwegian priority list that are less than 0,1 % by
weight.
The product contain dangerous substances, more then 0,1% by weight, given by the REACH Candidate List or the Norwegian
Priority list, see table.
The product contains no substances given by the REACH Candidate list or the Norwegian priority list. The product is classified
as hazardous waste (Avfallsforskiften, Annex III), see table.
Name CAS no. Amount
Lead 7439-92-1 0,1% - 2,4% (in brass alloys)
indoor environment
The product meets the requirements for low emissions according to EN15251: 2007 Appendix E.
No tests have been carried out on the product concerning indoor climate - Not relevant
carbon footprint
Carbon footprint has not been worked out for the product
NEPD-2147-970-EN Product-specific Type III EPD of Cimberio valves (ver2-200421) 7/8
Bibliography
ISO 14025:2010 Environmental labels and declarations - Type III environmental declarations - Principles and
procedures
ISO 14044:2006 Environmental management - Life cycle assessment - Requirements and guidelines
EN 15804:2012+A2:2019 Sustainability of construction works. Environmental product declarations. Core rules for the
product category of construction products
PCR Product Category Rules “Products and Services - Part B: Requirements on the EPD for
Bathroom fittings and showers”.
LCI Report Cimberio LCI / LCA Report – A2life
Ecoinvent center Ecoinvent v. 3.6
program operator
The Norwegian EPD Foundation phone: +47 23 08 82 92
Post Box 5250 Majorstuen, 0303 Oslo e-mail: post@epd-norge.no
Norway web: www.epd-norge.no
publisher
The Norwegian EPD Foundation phone: +47 23 08 82 92
Post Box 5250 Majorstuen, 0303 Oslo e-mail: post@epd-norge.no
Norway web: www.epd-norge.no
owner of the declaration
Cav. Uff. Giacomo Cimberio S.p.A. phone: +39 0322 923001
Via Torchio, 57- C.P. 106 - e-mail: info@cimberio.it
28017, San Maurizio d’Opaglio, Italy web: www.cimberio.com/index.asp
author of the life cycle assessment
Arch. Ph.D. Sara Ganassali / A2life phone: +39 0371 431558
Via Sobacchi 20 e-mail: sara.ganassali@a2life-sg.com
26900, Lodi, Italy web: www.saraganassaliarchitetto.com
NEPD-2147-970-EN Product-specific Type III EPD of Cimberio valves (ver2-200421) 8/8
