Environmental product declaration
in accordance with ISO 14025 and EN 15804+A2
Optima TS0101, Outward opening, Topguided window, Wood with 2-layer insulated
glass unit.
Owner of the declaration: Program operator:
JABS Group A/S The Norwegian EPD Foundation
Product: Declaration number:
Optima TS0101, Outward opening, Topguided window,
Wood with 2-layer insulated glass unit. NEPD-8983-8647
Declared unit: Registration number:
1 pcs
NEPD-8983-8647
This declaration is based on Product Category Rules:
Issue date: 06.02.2025
CEN Standard EN 15804:2012+A2:2019 serves as core
The Norwegian EPD Foundation PCR Valid to: 06.02.2030
NPCR 014:2019 Part B for Windows and doors
EPD software:
LCAno EPD generator ID: 777172
1 / 13
General information
Product Owner of the declaration:
Optima TS0101, Outward opening, Topguided window, Wood with 2- JABS Group A/S
layer insulated glass unit. Contact person: Henrik Bonde Hanfgarn
Phone: +45 70201887
e-mail: sustainability@jabsgroup.com
Program operator: Manufacturer:
The Norwegian EPD Foundation JABS Group A/S
Post Box 5250 Majorstuen, 0303 Oslo, Norway Cortex Park 3
Phone: +47 977 22 020 5230 Odense, Denmark
web: www.epd-norge.no
Declaration number: Place of production:
JABS Group:
NEPD-8983-8647
Romania, Poland, Estonia
, Europe
This declaration is based on Product Category Rules: Management system:
CEN Standard EN 15804:2012+A2:2019 serves as core PCR
NPCR 014:2019 Part B for Windows and doors
Statement of liability: Organisation no:
The owner of the declaration shall be liable for the underlying 37416258
information and evidence. EPD Norway shall not be liable with respect
to manufacturer information, life cycle assessment data and
evidences.​
Declared unit: Issue date:
1 pcs Optima TS0101, Outward opening, Topguided window, Wood
06.02.2025
with 2-layer insulated glass unit.
Declared unit with option: Valid to:
A1-A3,A4,A5,B2,B4,C1,C2,C3,C4,D
06.02.2030
Year of study:
2023
Functional unit: Comparability:
1 installed wood window with a 2-layer insulated glass unit, designed EPD of construction products may not be comparable if they not
to provide thermal insulation, natural lighting, and ventilation. 1.23 m comply with EN 15804 and seen in a building context.
x 1.48m reference window based on EN 14351-1
General information on verification of EPD from EPD tools: Development and verification of EPD:
Independent verification of data, other environmental information The declaration is created using EPD tool lca.tools ver EPD2022.03,
and the declaration according to ISO 14025:2010, § 8.1.3 and § 8.1.4. developed by LCA.no. The EPD tool is integrated in the company's
Verification of each EPD is made according to EPD-Norway’s management system, and has been approved by EPD Norway.
guidelines for verification and approval requiring that tools are i) NEPDT139
integrated into the company's environmental management system, ii)
the procedures for use of the EPD tool are approved by EPD-Norway, Developer of EPD: Kadri-Ann Jundas
and iii) the process is reviewed annually by an independent third
Reviewer of company-specific input data and EPD:​ Erik Tamm
party verifier. See Appendix G of EPD-Norway's General Programme
Instructions for further information on EPD tools
Verification of EPD tool: Approved:
Independent third party verification of the EPD tool, background data
and test-EPD in accordance with EPDNorway's procedures and
guidelines for verification and approval of EPD tools.
Third party verifier:
Gaylord K. Booto, Norwegian Institute for Air Research (NILU)
(no signature required)
2 / 13
Product
Product description:
Window with outward opening sash for use in exterior walls of domestic and commercial buildings
Product specification
Wood with 2-layer insulated glass unit
Materials kg %
Glass - coated 29,00 48,66
Metal - Alloy 0,10 0,17
Metal - Galvanized Steel 0,14 0,23
Paint, water-based 2,55 4,28
Plastic - Polyoxymethylene (POM) 0,01 0,01
Plastic - Polypropylene (PP) 0,13 0,22
Rubber, synthetic 0,41 0,68
Metal 0,21 0,35
Metal - Aluminium 0,71 1,20
Metal - Zamak 0,57 0,96
Tape 0,08 0,13
Polyethylene (LDPE) 0,10 0,17
Wood - Laminated wood 25,60 42,95
Total 59,60 100,00
Packaging kg %
Packaging - Wood 4,00 100,00
Total incl. packaging 63,60 100,00
Technical data:
Glazing composition: 4-X-4 configuration. Frame profile dimensions: 44 mm. x 116 mm., providing structural stability and improved thermal
performance. Surface treatment: Factory-applied water-based paint for increased resistance to moisture and weathering, ensuring longevity and
low maintenance.
Market:
We proudly sell to, and care for customers across Europe. Scenarios beyond cradle-to-gate are based on the situation in the Danish market.
Reference service life, product
The Reference Service Life (RSL) is estimated at 40 years under typical usage and environmental conditions. Actual lifespan may vary depending on
climate, exposure, installation quality, and maintenance. Regular upkeep is recommended to maximize performance and durability.
Reference service life, building or construction works
60
LCA: Calculation rules
Declared unit:
1 pcs Optima TS0101, Outward opening, Topguided window, Wood with 2-layer insulated glass unit.
Cut-off criteria:
All major raw materials and all the essential energy is included. The production processes for raw materials and energy flows with very small
amounts (less than 1%) are not included. These cut-off criteria do not​ apply for hazardous materials and substances.
Allocation:
The allocation is made in accordance with the provisions of EN 15804. Effects of primary production of recycled materials is allocated to the main
product in which the material was used. The recycling process and transportation of the material is allocated to this analysis. The PCR specific
background data follow the allocation rules in the Ecoinvent v3.7.1 Cut-off database version. The allocation of water, energy and waste flows
within the production facilities for windows and doors follows unit-based allocation adjusted with a point system to different product groups or
products. This score system is regulated by a factor which increases with the resource intensity of each product. The unit-based allocation is
adjusted by the weight of the product, excluding the weight of glass.
Data quality:
Specific data for the product composition are provided by the manufacturer. The data represent the production of the declared product and were
collected for EPD development in the year of study. Background data is based on EPDs according to EN 15804 and different LCA databases. The
data quality of the raw materials in A1 is presented in the table below.
3 / 13
Materials Source Data quality Year
Glass - coated S-P-09512 EPD 2019
Metal EPD-ARG-20230542-IBG1-EN EPD 2022
Metal - Alloy ecoinvent 3.6 Database 2019
Metal - Aluminium S-P-07377 EPD 2021
Metal - Galvanized Steel Ecoinvent 3.6 Database 2019
Metal - Zamak EPD-ARG-20230541-IBG1-EN EPD 2022
Packaging - Wood Modified ecoinvent 3.6 Database 2019
Paint, water-based ecoinvent 3.6 Database 2019
Plastic - Polyoxymethylene (POM) ecoinvent 3.6 Database 2019
Plastic - Polypropylene (PP) ecoinvent 3.6 Database 2019
Polyethylene (LDPE) ecoinvent 3.6 Database 2019
Rubber, synthetic ecoinvent 3.6 Database 2019
Tape ecoinvent 3.6 Database 2019
Wood - Laminated wood EPD HUB, HUB-0102 EPD 2021
4 / 13
System boundaries (X=included, MND=module not declared, MNR=module not relevant)
Construction Beyond the system
Product stage Use stage End of life stage
installation stage boundaries
A1 A2 A3 A4 A5 B1 B2 B3 B4 B5 B6 B7 C1 C2 C3 C4 D
X X X X X MND X MND X MND MND MND X X X X X
System boundary:
Additional technical information:
The wood raw material used is pine supplied by FSC or PEFC-labelled suppliers, that glues and finger joint wood raw material. The wood is cut and
planed and processed at the production site. The finished wood details are surface treated with a water-based paint system.
JABS Group uses IGU's produced by Europe's largest glass manufacturers.
waR slairetam tropsnarT gnirutcafunaM tropsnarT ylbmessA e​sU ecnanetniaM riapeR tnemecalpeR tnemhsibrufeR lanoitarepO ygrene esu lanoitarepO esu retaw -eD noitcurtsnoc noitilomed tropsnarT etsaW gnissecorp lasopsiD -yrevoceR-esueR laitnetop-gnilcyceR
5 / 13
LCA: Scenarios and additional technical information
The following information describe the scenarios in the different modules of the EPD.
Average or specific EPD: Average.
This EPD is averaged for the production, in regard to the production sites. Production is done by JABS Group production sites, all part of JABS
Group. Production is taking place in Estonia, Poland and Romania. An average weighted number is presented in the results based on the
production from the different sites.
A4: Transportation - FTL sent from factory, with an average of 90 units per trailer. Transported to terminal by Road, truck, EURO 6, 16-32
tons/ferry/road. Distributed to customer - average distance from DC 160 km. The finished windows and doors are packed on a wooden pallet and
transported by truck to the customer.
We have utilized extensive data from our operations in Denmark to calculate average scenarios related to the delivery phase for our
Environmental Product Declarations (EPDs) on windows and doors. This allows us to create the most accurate representations of the
environmental impacts associated with transportation, ensuring our EPDs reflect realistic, region-specific delivery conditions.
A5: Installation - Our products are painted and surface-treated during the production. Therefore, there is left waste treatment of packaging which
is considered in the EPD calculations and energy use during installation.
B2: Maintenance - The maintenance scenario includes cleaning, painting and maintenance change of IGU. The product is assumed to require
0.15kg/unit soap or detergent and 3 kg/unit water per year. The product is expected to be painted 1-2 times from inside and 4 times from outside
which take 0.0325kg/unit paint, during product lifetime. It's assumed to require 0.05 kg/unit of lubricating oil for fittings and moving parts per
year.
C1: Removal - Removing the window frame and glass consume a small amount of electricity. Estimated 1-2 Kwh.
Capacity utilisation Value
Transport from production place to user (A4) Distance (km) Fuel/Energy Consumption Unit
(incl. return) % (Liter/tonne)
Truck, 16-32 tonnes, EURO 6 (km) - Europe 36,7 % 160 0,043 l/tkm 6,88
Assembly (A5) Unit Value
Waste, packaging, pallet, EUR wooden pallet,
kg 4,000000000
reusable, average treatment (kg)
Maintenance (B2) Unit Value
Treatment of wastewater (kg) kg 126,000000000
Lubricant (kg) kg 0,20
Water, tap water (kg) kg 120,000000000
Soap solution 5%, household detergent (kg) -
kg 6,000000000
pure soap
Replacement (B4) Unit Value
Replace product, including waste treatment (psc) Units 0,33
De-construction demolition (C1) Unit Value
Electricity, Estonia (kWh) kWh 1,000000000
Waste processing (C3) Unit Value
Waste treatment per kg Plastic, Mixture,
kg 0,071
municipal incineration with fly ash extraction (kg)
Waste treatment per kg Polypropylene, PP,
kg 0,12
incineration with fly ash extraction - C3 (kg)
Waste treatment per kg Wood, from incineration
kg 24,31
(kg)
Waste treatment per kg Paint, hazardous waste
kg 2,42
incineration (kg)
Waste treatment per kg Sealing sheet,
Polyethylene (PE), incineration with fly ash kg 0,095
extraction (kg)
Materials to recycling (kg) kg 10,34
Waste treatment per kg Rubber, municipal
kg 0,38
incineration with fly ash extraction (kg)
Waste treatment per kg Polyoxymethylene
(POM), incineration with fly ash extraction (kg) - kg 0,0047
CH - C3
6 / 13
Disposal (C4) Unit Value
Waste, scrap steel, to landfill (kg) kg 0,050
Landfilling of ashes from incineration of
Polyoxymethylene (POM), process per kg ashes kg 0,00010
and residues (kg) - CH - C4
Waste, rubber, to landfill (kg) kg 0,024
Waste, scrap aluminium, to landfill (kg) kg 0,035
Waste, glass, to landfill (kg) kg 20,30
Waste, paint, to landfill (kg) kg 0,12
Landfilling of ashes from incineration of Wood,
kg 0,27
process per kg ashes and residues - C4 (kg)
Waste, polyethylene, to landfill (kg) kg 0,0050
Landfilling of ashes from incineration per kg
Sealing sheet, Polyethylene (PE), process per kg kg 0,019
ashes and residues (kg)
Landfilling of ashes from incineration of
Polypropylene, PP, process per kg ashes and kg 0,0036
residues - C4 (kg)
Waste, Polyoxymethylene (POM), to landfill (kg) kg 0,00025
Landfilling of ashes from incineration of Rubber,
kg 0,020
process per kg ashes and residues - C4 (kg)
Landfilling of ashes from incineration of Plastics,
Mixture, municipal incineration with fly ash
kg 0,0024
extraction, process per kg ashes and residues - C4
(kg)
Waste, polypropylene, to landfill (kg) kg 0,0064
Landfilling of ashes from incineration of Paint,
hazardous waste incineration, process of ashes kg 0,071
and residues (kg)
Waste, wood, untreated, to landfill (kg) kg 1,27
Benefits and loads beyond the system
Unit Value
boundaries (D)
Substitution of primary steel with net scrap (kg) kg 0,85
Substitution of electricity (MJ) MJ 17,91
Substitution of primary aluminium with net scrap
kg 0,67
(kg)
Substitution of electricity (MJ) MJ 0,13
Substitution of thermal energy (MJ) MJ 270,97
Substitution of thermal energy, district heating
MJ 2,087
(MJ)
7 / 13
LCA: Results
The LCA results are presented below for the declared unit defined on page 2 of the EPD document.
Environmental impact
Indicator Unit A1-A3 A4 A5 B2 B4 C1 C2 C3 C4 D
GWP-total
kg CO2 -
5,00E+01 1,66E+00 6,07E+00 1,99E+00 3,68E+01 9,27E-01 0 5,24E+01 3,65E-01 -8,74E+00
eq
GWP-fossil
kg CO2 -
9,42E+01 1,66E+00 5,38E-03 9,24E-01 3,54E+01 9,25E-01 0 1,01E+01 2,55E-01 -8,54E+00
eq
GWP-biogenic
kg CO2 -
-4,75E+01 6,88E-04 6,06E+00 1,29E-01 3,01E-01 1,31E-03 0 4,23E+01 1,10E-01 -3,14E-02
eq
GWP-luluc
kg CO2 -
3,27E+00 5,92E-04 1,38E-06 9,34E-01 1,08E+00 7,84E-04 0 7,94E-04 6,47E-05 -1,69E-01
eq
kg
ODP CFC11 - 1,13E-05 3,76E-07 8,60E-10 2,58E-07 4,11E-06 1,75E-07 0 5,03E-07 7,26E-08 -1,15E-01
eq
mol H+
AP 7,84E-01 4,78E-03 4,33E-05 1,02E-02 2,67E-01 8,57E-03 0 1,09E-02 1,94E-03 -5,84E-02
-eq
EP-FreshWater kg P -eq 5,12E-02 1,33E-05 6,45E-08 4,91E-03 1,69E-02 1,02E-05 0 1,78E-05 3,01E-06 -4,31E-04
EP-Marine kg N -eq 1,26E-01 9,45E-04 1,86E-05 1,07E-02 4,35E-02 1,20E-03 0 3,19E-03 7,37E-04 -1,04E-02
mol N -
EP-Terrestial 1,50E+00 1,06E-02 1,99E-04 3,06E-02 5,16E-01 1,34E-02 0 3,52E-02 7,42E-03 -1,13E-01
eq
kg
POCP NMVOC 3,88E-01 4,05E-03 5,11E-05 9,86E-03 1,35E-01 4,12E-03 0 1,00E-02 2,16E-03 -3,65E-02
-eq
ADP- kg Sb-
1,20E-02 4,59E-05 8,73E-08 6,11E-05 3,97E-03 2,45E-06 0 8,05E-06 2,35E-06 -2,27E-05
minerals&metals1 eq
ADP-fossil1 MJ 1,40E+03 2,51E+01 6,32E-02 1,96E+01 4,86E+02 1,29E+01 0 3,22E+01 5,30E+00 -1,07E+02
WDP1 m3 7,06E+03 2,43E+01 9,74E-02 7,34E+01 2,43E+03 1,19E+02 0 1,35E+02 7,90E+00 -3,68E+03
GWP-total = Global Warming Potential total; GWP-fossil = Global Warming Potential fossil fuels; GWP-biogenic = Global Warming Potential biogenic; GWP-luluc =
Global Warming Potential land use and land use change; ODP = Depletion potential of the stratospheric ozone layer; AP = Acidification potential, Accumulated
Exceedance; EP-freshwater = Eutrophication potential, fraction of nutrients reaching freshwater end compartment: EP-marine = Eutrophication potential, fraction of
nutrients reaching marine end compartment; EP-terrestrial = Eutrophication potential, Accumulated Exceedance; POCP = Formation potential of tropospheric ozone;
ADP-minerals&metals = Abiotic depletion potential for non-fossil resources; ADP-fossil = Abiotic depletion for fossil resources potential; WDP = Water (user)
deprivation potential, deprivation-weighted water consumption
"Reading example: 9,0 E-03 = 9,0*10-3 = 0,009"
*INA Indicator Not Assessed
1. The results of this environmental impact indicator shall be used with care as the uncertainties on these results are high or as there is limited experienced with the
indicator
Remarks to environmental impacts
8 / 13
Additional environmental impact indicators
Indicator Unit A1-A3 A4 A5 B2 B4 C1 C2 C3 C4 D
PM Disease incidence 3,78E-06 1,02E-07 5,28E-10 1,28E-07 1,38E-06 6,90E-08 0 2,04E-07 3,77E-08 -1,29E-06
IRP2 kgBq U235 -eq 2,53E+00 1,10E-01 2,29E-04 7,83E-02 9,56E-01 9,14E-02 0 1,47E-01 2,13E-02 -4,74E-01
ETP-fw1 CTUe 1,74E+03 1,86E+01 7,20E-02 1,09E+02 6,04E+02 1,04E+01 0 4,06E+01 2,61E+01 -2,66E+02
HTP-c1 CTUh 9,31E-08 0,00E+00 8,00E-12 2,18E-09 3,71E-08 1,22E-09 0 1,79E-08 1,63E-10 -2,20E-08
HTP-nc1 CTUh 2,50E-06 2,03E-08 3,84E-10 5,21E-08 8,60E-07 5,67E-09 0 7,49E-08 3,51E-09 -1,97E-07
SQP1 dimensionless 7,80E+02 1,76E+01 3,55E-02 3,97E+01 2,75E+02 7,29E+00 0 1,58E+01 1,44E+01 -1,53E+02
PM = Particulate Matter emissions; IRP = Ionizing radiation – human health; ETP-fw = Eco toxicity – freshwater; HTP-c = Human toxicity – cancer effects; HTP-nc =
Human toxicity – non cancer effects; SQP = Potential Soil Quality Index (dimensionless)
"Reading example: 9,0 E-03 = 9,0*10-3 = 0,009"
*INA Indicator Not Assessed
1. The results of this environmental impact indicator shall be used with care as the uncertainties on these results are high or as there is limited experienced with the
indicator
2. This impact category deals mainly with the eventual impact of low dose ionizing radiation on human health of the nuclear fuel cycle. It does not consider effects due
to possible nuclear accidents, occupational exposure nor due to radioactive waste disposal in underground facilities. Potential ionizing radiation from the soil, from
radon and from some construction materials is also not measured by this indicator.
9 / 13
Resource use
Indicator Unit A1-A3 A4 A5 B2 B4 C1 C2 C3 C4 D
PERE MJ 6,21E+02 3,60E-01 1,30E-03 9,41E+00 2,08E+02 1,83E+00 0 6,78E+00 8,57E-02 -1,68E+02
PERM MJ 3,01E+02 0,00E+00 -5,55E+01 0,00E+00 -1,36E-09 0,00E+00 0 -2,46E+02 0,00E+00 0,00E+00
PERT MJ 9,22E+02 3,60E-01 -5,55E+01 9,41E+00 2,08E+02 1,83E+00 0 -2,39E+02 8,57E-02 -1,68E+02
PENRE MJ 1,38E+03 2,51E+01 6,32E-02 2,09E+01 4,80E+02 1,30E+01 0 3,22E+01 5,30E+00 -1,07E+02
PENRM MJ 4,00E+01 0,00E+00 0,00E+00 0,00E+00 1,68E-09 0,00E+00 0 -4,00E+01 0,00E+00 0,00E+00
PENRT MJ 1,42E+03 2,51E+01 6,32E-02 2,09E+01 4,80E+02 1,30E+01 0 -7,79E+00 5,30E+00 -1,07E+02
SM kg 1,65E-01 0,00E+00 0,00E+00 0,00E+00 5,44E-02 0,00E+00 0 0,00E+00 0,00E+00 0,00E+00
RSF MJ 6,58E+00 1,29E-02 3,79E-05 3,31E-02 2,23E+00 3,04E-02 0 1,41E-01 1,80E-03 -1,84E-03
NRSF MJ 5,45E-01 4,60E-02 4,32E-04 2,51E-02 2,47E-01 1,80E-02 0 0,00E+00 1,39E-01 -7,26E+00
FW m3 1,50E+00 2,69E-03 4,60E-05 1,13E-01 5,03E-01 3,94E-03 0 1,19E-02 5,75E-03 -3,22E-01
PERE = Use of renewable primary energy excluding renewable primary energy resources used as raw materials; PERM = Use of renewable primary energy resources used
as raw materials; PERT = Total use of renewable primary energy resources; PENRE = Use of non renewable primary energy excluding non-renewable primary energy
resources used as raw materials; PENRM = Use of non renewable primary energy resources used as raw materials; PENRT = Total use of non renewable primary energy
resources; SM = Use of secondary materials; RSF = Use of renewable secondary fuels; NRSF = Use of non-renewable secondary fuels; FW = Net use of fresh water
"Reading example: 9,0 E-03 = 9,0*10-3 = 0,009"
*INA Indicator Not Assessed
10 / 13
End of life - Waste
Indicator Unit A1-A3 A4 A5 B2 B4 C1 C2 C3 C4 D
HWD kg 4,81E+01 1,30E-03 0,00E+00 9,91E-02 1,60E+01 8,45E-04 0 0,00E+00 2,39E-01 1,94E-02
NHWD kg 2,42E+01 1,22E+00 2,00E-01 3,04E-01 1,58E+01 2,37E-02 0 0,00E+00 2,21E+01 -2,67E+00
RWD kg 2,16E-02 1,71E-04 0,00E+00 9,91E-05 7,22E-03 9,34E-05 0 0,00E+00 3,22E-06 -4,29E-04
HWD = Hazardous waste disposed; NHWD = Non-hazardous waste disposed; RWD = Radioactive waste disposed
"Reading example: 9,0 E-03 = 9,0*10-3 = 0,009"
*INA Indicator Not Assessed
End of life - Output flow
Indicator Unit A1-A3 A4 A5 B2 B4 C1 C2 C3 C4 D
CRU kg 0,00E+00 0,00E+00 3,80E+00 0,00E+00 1,25E+00 0,00E+00 0 0,00E+00 0,00E+00 0,00E+00
MFR kg 9,16E+00 0,00E+00 4,69E-06 0,00E+00 6,44E+00 0,00E+00 0 1,03E+01 1,15E-04 0,00E+00
MER kg 7,84E-01 0,00E+00 1,98E-01 0,00E+00 8,57E+00 0,00E+00 0 2,50E+01 2,37E-06 0,00E+00
EEE MJ 4,93E-01 0,00E+00 1,38E-01 0,00E+00 6,12E+00 0,00E+00 0 1,79E+01 1,80E-04 0,00E+00
EET MJ 7,46E+00 0,00E+00 2,09E+00 0,00E+00 9,26E+01 0,00E+00 0 2,71E+02 2,72E-03 0,00E+00
CRU = Components for re-use; MFR = Materials for recycling; MER = Materials for energy recovery; EEE = Exported energy electrical; EET = Exported energy thermal
"Reading example: 9,0 E-03 = 9,0*10-3 = 0,009"
*INA Indicator Not Assessed
Biogenic Carbon Content
Indicator Unit At the factory gate
Biogenic carbon content in product kg C 1,15E+01
Biogenic carbon content in accompanying packaging kg C 1,65E+00
Note: 1 kg biogenic carbon is equivalent to 44/12 kg CO2
11 / 13
Additional requirements
Greenhouse gas emissions from the use of electricity in the manufacturing phase
National production mix from import, low voltage (production of transmission lines, in addition to direct emissions and losses in grid) of applied
electricity for the manufacturing process (A3).
Electricity mix Source Amount Unit
Electricity, Estonia (kWh) ecoinvent 3.6 926,93 g CO2-eq/kWh
Electricity, with Guarantee of origin, 2023, Goldeni, Romania (kWh) Modified ecoinvent 3.6 145,05 g CO2-eq/kWh
Electricity, low voltage, biogas, wind, solar and hydro based, 2023, Sokolka, Poland (kWh) Modified ecoinvent 3.6 67,19 g CO2-eq/kWh
Dangerous substances
The product contains no substances given by the REACH Candidate list.
Indoor environment
No negative impact. A new window or door can improve energy efficiency, reduces heating and cooling costs, minimizes noise.
Additional Environmental Information
Additional environmental impact indicators required in NPCR Part A for construction products
Indicator Unit A1-A3 A4 A5 B2 B4 C1 C2 C3 C4 D
GWPIOBC kg CO2 -eq 1,00E+02 1,66E+00 5,38E-03 1,98E+00 3,74E+01 1,03E+00 0 1,02E+01 3,66E-01 -8,90E+00
GWP-IOBC: Global warming potential calculated according to the principle of instantaneous oxidation. In order to increase the transparency of biogenic carbon​
contribution to climate impact, the indicator GWP-IOBC is required as it declares climate impacts calculated according to the principle of instantaneous oxidation.​
GWP-IOBC is also referred to as GWP-GHG in context to Swedish public procurement legislation.
12 / 13
Bibliography
ISO 14025:2010 Environmental labels and declarations - Type III environmental declarations - Principles and procedures.
ISO 14044:2006 Environmental management - Life cycle assessment - Requirements and guidelines.
EN 15804:2012+A2:2019 Environmental product declaration - Core rules for the product category of construction products.
ISO 21930:2017 Sustainability in buildings and civil engineering works - Core rules for environmental product declarations of construction
products.
ecoinvent v3, Allocation, cut-off by classification, Swiss Centre of Life Cycle Inventories.
Iversen et al., (2021) eEPD v2021.09 Background information for EPD generator tool system verification, LCA.no Report number: 07.21
Iversen et al., (2022) EPD generator for EPD generator for NPCR 014
Part B for Windows and doors, Background information for EPD generator application and LCA data, LCA.no report number: 17.22
NPCR Part A: Construction products and services. Ver. 2.0. April 2021, EPD-Norge.
NPCR 014 Part B for Windows and doors, Ver. 4.0, 20.09.2021, EPD Norway.
Program operator and publisher Phone: +47 977 22 020
The Norwegian EPD Foundation e-mail: post@epd-norge.no
Post Box 5250 Majorstuen, 0303 Oslo, Norway web: www.epd-norge.no
Owner of the declaration: Phone: +45 70201887
JABS Group A/S e-mail: sustainability@jabsgroup.com
Cortex Park 3, 5230 Odense, Denmark web: www.jabsgroup.com
Author of the Life Cycle Assessment Phone: +47 916 50 916
LCA.no AS e-mail: post@lca.no
Dokka 6A, 1671 Kråkerøy, Norway web: www.lca.no
Developer of EPD generator Phone: +47 916 50 916
LCA.no AS e-mail: post@lca.no
Dokka 6A, 1671 Kråkerøy, Norway web: www.lca.no
ECO Platform web: www.eco-platform.org
ECO Portal web: ECO Portal
13 / 13
