Environmental product declaration
in accordance with ISO 14025 and EN 15804+A2
EST170-C43L
Owner of the declaration: Program operator:
Maxeta AS The Norwegian EPD Foundation
Product: Declaration number:
EST170-C43L
NEPD-7994-7658-EN
Declared unit:
1 pcs Registration number:
This declaration is based on Product Category Rules: NEPD-7994-7658-EN
CEN Standard EN 15804:2012+A2:2019, EN
Issue date: 08.11.2024
50693:2019, EPDItaly007 serves as core PCR
PCR EPD Italy 10 - Insulators Valid to: 08.11.2029
The Norwegian EPD Foundation EPD software:
LCAno EPD generator ID: 495067
1 / 11
General information
Product Owner of the declaration:
EST170-C43L Maxeta AS
Contact person: Eivind Portaas Walstad
Phone:
e-mail: maxeta@maxeta.no
Program operator: Manufacturer:
The Norwegian EPD Foundation Pfisterer
Post Box 5250 Majorstuen, 0303 Oslo, Norway Rosenstrasse 44
Phone: +47 977 22 020 73650 Winterbach, Germany
web: www.epd-norge.no
Declaration number: Place of production:
Pfisterer production site (Czech Republic)
NEPD-7994-7658-EN
Královský Vrch 1977
43201 Kadan , Czech Republic
This declaration is based on Product Category Rules: Management system:
CEN Standard EN 15804:2012+A2:2019, EN 50693:2019,
EPDItaly007 serves as core PCR
PCR EPD Italy 10 - Insulators
Statement of liability: Organisation no:
The owner of the declaration shall be liable for the underlying 864 425 402
information and evidence. EPD Norway shall not be liable with respect
to manufacturer information, life cycle assessment data and
evidences.​
Declared unit: Issue date:
1 pcs EST170-C43L
08.11.2024
Declared unit with option: Valid to:
A1-A3,A4,A5,C1,C2,C3,C4,D 08.11.2029
Year of study:
2023
Functional unit: Comparability:
1 pc. Outdoor termination EST170-C43L, Dry-insulated 170kV. The EPD for electronic and electrical products and systems may not be
EST is fitted to the cable whilst on the ground and subsequently comparable if they do not comply with similar PCR standards
raised up onto the pylon. No mounting frame is required. The
assembe time is minimised.
General information on verification of EPD from EPD tools: Development and verification of EPD:
Independent verification of data, other environmental information The declaration is created using EPD tool lca.tools ver EPD2022.03,
and the declaration according to ISO 14025:2010, § 8.1.3 and § 8.1.4. developed by LCA.no. The EPD tool is integrated in the company's
Verification of each EPD is made according to EPD-Norway’s management system, and has been approved by EPD Norway.
guidelines for verification and approval requiring that tools are i)
integrated into the company's environmental management system, ii) Developer of EPD: Andreas Johnsen
the procedures for use of the EPD tool are approved by EPD-Norway,
Reviewer of company-specific input data and EPD:​ Nathaniel Kittilsen
and iii) the process is reviewed annually by an independent third
Aale
party verifier. See Appendix G of EPD-Norway's General Programme
Instructions for further information on EPD tools
Verification of EPD tool: Approved:
Independent third party verification of the EPD tool, background data
and test-EPD in accordance with EPDNorway's procedures and
guidelines for verification and approval of EPD tools.
Third party verifier:
Elisabet Amat, GREENIZE projects
(no signature required)
2 / 11
Product
Product description:
With the new EST dry outdoor termination, PFISTERER offers a self-supporting, dry and compact termination up to 170 kV. It reliably connects
cable systems with overhead lines and busbars in maintenance-free long-term use. The EST self-supporting outdoor termination meets all criteria
of the highest pollution class according to IEC 60815-3.
Expected service life after installation 40 years.
Product specification
EST170-C43L weight approx 152 kg
During the transportation, the product will weigh approximately 185 kg.
Materials kg %
Epoxy Resin 6,48 3,54
Metal - Aluminium 51,06 27,93
Silicone 95,29 52,12
Total 152,83 83,59
Packaging kg %
Packaging - Wood 30,00 16,41
Total incl. packaging 182,83 16,41
Technical data:
Datasheet: https://catalogue.pfisterer.com/en/est170-c43l/
General information: https://catalogue.pfisterer.com/en/connections-52-550-kv/cable-accessories/cable-terminations/
Market:
Norway
Reference service life, product
40 years.
Reference service life, building or construction works
N/A
LCA: Calculation rules
Declared unit:
1 pcs EST170-C43L
Cut-off criteria:
All major raw materials and all the essential energy is included. The production processes for raw materials and energy flows with very small
amounts (less than 1%) are not included. These cut-off criteria do not​ apply for hazardous materials and substances.
Allocation:
The allocation is made in accordance with the provisions of EN 15804. Incoming energy and water and waste production in-house is allocated
equally among all products through mass allocation. Effects of primary production of recycled materials is allocated to the main product in which
the material was used. The recycling process and transportation of the material is allocated to this analysis.
Data quality:
Specific data for the product composition are provided by the manufacturer. The data represent the production of the declared product and were
collected for EPD development in the year of study. Background data is based on EPDs according to EN 15804 and different LCA databases. The
data quality of the raw materials in A1 is presented in the table below.
Materials Source Data quality Year
Epoxy Resin Ecoinvent 3.6 Database 2019
Metal - Aluminium ecoinvent 3.6 Database 2019
Packaging - Wood ecoinvent 3.6 Database 2019
Silicone ecoinvent 3.6 Database 2019
3 / 11
System boundaries (X=included, MND=module not declared, MNR=module not relevant)
Construction Beyond the system
Product stage Use stage End of life stage
installation stage boundaries
A1 A2 A3 A4 A5 B1 B2 B3 B4 B5 B6 B7 C1 C2 C3 C4 D
X X X X X MND MND MND MND MND MND MND X X X X X
System boundary:
The system includes the production of raw materials (A1), the transport of these raw materials to manufacturing facility (A2), manufacturing with
raw material preparation, cold pressing, drying, firing, and glazing (A3), transport to market (A4), installation (A5), and end-of-life stages (C1-C4,
D).
Additional technical information:
waR slairetam tropsnarT gnirutcafunaM tropsnarT ylbmessA e​sU ecnanetniaM riapeR tnemecalpeR tnemhsibrufeR lanoitarepO ygrene esu lanoitarepO esu retaw -eD noitcurtsnoc noitilomed tropsnarT etsaW gnissecorp lasopsiD -yrevoceR-esueR laitnetop-gnilcyceR
4 / 11
LCA: Scenarios and additional technical information
The following information describe the scenarios in the different modules of the EPD.
Module A4 = Includes the transport from the factory to the end customer in Norway.
Module A5 = Includes installation of the product done via manual installation and disposal of packaging.
Module C1 = Includes disassembly of the product done via manual disassembly . Falls under the 1% cutoff criteria and therefore excluded from
the inputs.
Module C2 = Transport to average recycling station in Norway.
Modules C3 and C4 = Waste treatment of the product follows the default values provided in EN 50693, Product Category Rules for life cycle
assessments of electronic and electrical products and systems, table G.4. This table specified how different types of raw materials used in A1 will
likely be treated during the end-of-life of the product. Waste treatments in C3 include material recycling and incineration with energy recovery and
fly ash extraction. Disposal in C4 consist of landfilling of different waste fractions and of ashes.
Module D = The recyclability of metals, plastics, and electronic components allows the producers a credit for the net scrap that is produced at the
end of a product’s life. The benefits from recycling of net scrap are described in formula from EN 15804:2012+A2:2019. Substitution of heat and
electricity generated by the incineration with energy recovery of plastic insulation and other parts is also calculated in module D.
Capacity utilisation Value
Transport from production place to user (A4) Distance (km) Fuel/Energy Consumption Unit
(incl. return) % (Liter/tonne)
Truck, 16-32 tonnes, EURO 5 (km) 36,7 % 1580 0,044 l/tkm 69,52
Assembly (A5) Unit Value
Waste, packaging, wood beam, softwood, raw,
dried, u=20%, average treatment (kg) - A5, inkl. 85 kg 30,00
km transp.
Capacity utilisation Value
Transport to waste processing (C2) Distance (km) Fuel/Energy Consumption Unit
(incl. return) % (Liter/tonne)
Truck, 16-32 tonnes, EURO 5 (km) 36,7 % 85 0,044 l/tkm 3,74
Waste processing (C3) Unit Value
Aluminium to recycling (kg) kg 35,74
Landfilling of ashes from incineration of Plastic
kg 50,88
mixture, process per kg ashes and residues (kg)
Waste treatment of plastic mixture, incineration
kg 50,88
with energy recovery and fly ash extraction (kg)
Disposal (C4) Unit Value
Landfilling of aluminium (kg) kg 15,32
Landfilling of ashes from incineration of Plastic
kg 1,78
mixture, process per kg ashes and residues (kg)
Benefits and loads beyond the system
Unit Value
boundaries (D)
Substitution of primary aluminium with net scrap
kg 35,74
(kg)
Substitution of electricity (MJ) MJ 78,18
Substitution of thermal energy, district heating
MJ 1182,75
(MJ)
5 / 11
LCA: Results
The LCA results are presented below for the declared unit defined on page 2 of the EPD document.
Environmental impact
Indicator Unit A1-A3 A4 A5 C1 C2 C3 C4 D
GWP-total kg CO2 -eq 9,00E+02 4,03E+01 4,66E+01 0 2,17E+00 1,21E+02 2,25E-01 -3,32E+02
GWP-fossil kg CO2 -eq 9,26E+02 4,02E+01 8,07E-01 0 2,17E+00 1,21E+02 2,25E-01 -3,24E+02
GWP-biogenic kg CO2 -eq -3,49E+01 1,64E-02 4,58E+01 0 8,83E-04 2,69E-03 2,57E-06 -1,47E+00
GWP-luluc kg CO2 -eq 9,44E+00 1,41E-02 2,07E-04 0 7,57E-04 5,08E-04 8,63E-05 -6,27E+00
ODP kg CFC11 -eq 2,24E-04 9,18E-06 1,29E-07 0 4,94E-07 2,74E-07 6,19E-08 -5,00E-01
AP mol H+ -eq 5,37E+00 1,65E-01 6,49E-03 0 8,85E-03 2,69E-02 1,72E-03 -2,21E+00
EP-FreshWater kg P -eq 4,31E-02 3,16E-04 9,68E-06 0 1,70E-05 2,52E-05 4,06E-06 -1,29E-02
EP-Marine kg N -eq 7,61E-01 4,88E-02 2,79E-03 0 2,63E-03 1,28E-02 6,17E-04 -2,90E-01
EP-Terrestial mol N -eq 8,44E+00 5,40E-01 2,98E-02 0 2,90E-02 1,31E-01 6,95E-03 -3,18E+00
POCP kg NMVOC -eq 2,87E+00 1,65E-01 7,67E-03 0 8,89E-03 3,16E-02 1,96E-03 -1,06E+00
ADP-minerals&metals1 kg Sb-eq 1,92E-02 1,09E-03 1,31E-05 0 5,87E-05 1,38E-05 1,70E-06 4,19E-04
ADP-fossil1 MJ 1,43E+04 6,07E+02 9,49E+00 0 3,26E+01 1,77E+01 5,11E+00 -4,13E+03
WDP1 m3 2,04E+05 5,79E+02 1,46E+01 0 3,11E+01 1,34E+02 1,32E+02 -1,83E+05
GWP-total = Global Warming Potential total; GWP-fossil = Global Warming Potential fossil fuels; GWP-biogenic = Global Warming Potential biogenic; GWP-luluc =
Global Warming Potential land use and land use change; ODP = Depletion potential of the stratospheric ozone layer; AP = Acidification potential, Accumulated
Exceedance; EP-freshwater = Eutrophication potential, fraction of nutrients reaching freshwater end compartment: EP-marine = Eutrophication potential, fraction of
nutrients reaching marine end compartment; EP-terrestrial = Eutrophication potential, Accumulated Exceedance; POCP = Formation potential of tropospheric ozone;
ADP-minerals&metals = Abiotic depletion potential for non-fossil resources; ADP-fossil = Abiotic depletion for fossil resources potential; WDP = Water (user)
deprivation potential, deprivation-weighted water consumption
"Reading example: 9,0 E-03 = 9,0*10-3 = 0,009"
*INA Indicator Not Assessed
1. The results of this environmental impact indicator shall be used with care as the uncertainties on these results are high or as there is limited experienced with the
indicator
Remarks to environmental impacts
6 / 11
Additional environmental impact indicators
Indicator Unit A1-A3 A4 A5 C1 C2 C3 C4 D
PM Disease incidence 5,02E-05 2,90E-06 7,94E-08 0 1,56E-07 1,21E-07 2,97E-08 -2,56E-05
IRP2 kgBq U235 -eq 6,28E+01 2,65E+00 3,44E-02 0 1,43E-01 4,72E-02 3,42E-02 -1,82E+01
ETP-fw1 CTUe 1,89E+04 4,47E+02 1,08E+01 0 2,40E+01 2,57E+02 9,48E+03 -5,32E+03
HTP-c1 CTUh 1,71E-06 0,00E+00 1,20E-09 0 0,00E+00 7,07E-09 4,33E-10 -8,13E-07
HTP-nc1 CTUh 2,50E-05 4,83E-07 5,77E-08 0 2,60E-08 3,22E-07 7,79E-09 -9,87E-06
SQP1 dimensionless 4,83E+03 4,18E+02 5,32E+00 0 2,25E+01 6,36E+00 8,91E+00 -6,90E+02
PM = Particulate Matter emissions; IRP = Ionizing radiation – human health; ETP-fw = Eco toxicity – freshwater; HTP-c = Human toxicity – cancer effects; HTP-nc =
Human toxicity – non cancer effects; SQP = Potential Soil Quality Index (dimensionless)
"Reading example: 9,0 E-03 = 9,0*10-3 = 0,009"
*INA Indicator Not Assessed
1. The results of this environmental impact indicator shall be used with care as the uncertainties on these results are high or as there is limited experienced with the
indicator
2. This impact category deals mainly with the eventual impact of low dose ionizing radiation on human health of the nuclear fuel cycle. It does not consider effects due
to possible nuclear accidents, occupational exposure nor due to radioactive waste disposal in underground facilities. Potential ionizing radiation from the soil, from
radon and from some construction materials is also not measured by this indicator.
7 / 11
Resource use
Indicator Unit A1-A3 A4 A5 C1 C2 C3 C4 D
PERE MJ 3,68E+03 8,56E+00 1,95E-01 0 4,61E-01 1,00E+00 7,12E-01 -2,07E+03
PERM MJ 4,20E+02 0,00E+00 -4,20E+02 0 0,00E+00 0,00E+00 0,00E+00 0,00E+00
PERT MJ 4,10E+03 8,56E+00 -4,20E+02 0 4,61E-01 1,00E+00 7,12E-01 -2,07E+03
PENRE MJ 1,33E+04 6,07E+02 9,49E+00 0 3,27E+01 1,77E+01 5,11E+00 -4,13E+03
PENRM MJ 9,43E+02 0,00E+00 0,00E+00 0 0,00E+00 -8,58E+02 0,00E+00 0,00E+00
PENRT MJ 1,43E+04 6,07E+02 9,49E+00 0 3,27E+01 -8,40E+02 5,11E+00 -4,13E+03
SM kg 0,00E+00 0,00E+00 0,00E+00 0 0,00E+00 0,00E+00 0,00E+00 0,00E+00
RSF MJ 1,99E+01 3,07E-01 5,69E-03 0 1,65E-02 2,17E-02 1,48E-02 -7,03E-01
NRSF MJ 3,75E+00 1,09E+00 6,48E-02 0 5,89E-02 1,83E-01 6,39E-03 -3,38E+01
FW m3 3,11E+01 6,39E-02 6,91E-03 0 3,44E-03 1,41E-01 6,69E-03 -8,71E+00
PERE = Use of renewable primary energy excluding renewable primary energy resources used as raw materials; PERM = Use of renewable primary energy resources used
as raw materials; PERT = Total use of renewable primary energy resources; PENRE = Use of non renewable primary energy excluding non-renewable primary energy
resources used as raw materials; PENRM = Use of non renewable primary energy resources used as raw materials; PENRT = Total use of non renewable primary energy
resources; SM = Use of secondary materials; RSF = Use of renewable secondary fuels; NRSF = Use of non-renewable secondary fuels; FW = Net use of fresh water
"Reading example: 9,0 E-03 = 9,0*10-3 = 0,009"
*INA Indicator Not Assessed
8 / 11
End of life - Waste
Indicator Unit A1-A3 A4 A5 C1 C2 C3 C4 D
HWD kg 4,39E+00 3,10E-02 0,00E+00 0 1,67E-03 1,35E+00 6,21E-01 1,33E+00
NHWD kg 1,70E+02 2,90E+01 3,00E+01 0 1,56E+00 1,29E+00 1,56E+01 -9,45E+01
RWD kg 5,79E-02 4,14E-03 0,00E+00 0 2,23E-04 6,71E-06 3,57E-05 -1,70E-02
HWD = Hazardous waste disposed; NHWD = Non-hazardous waste disposed; RWD = Radioactive waste disposed
"Reading example: 9,0 E-03 = 9,0*10-3 = 0,009"
*INA Indicator Not Assessed
End of life - Output flow
Indicator Unit A1-A3 A4 A5 C1 C2 C3 C4 D
CRU kg 0,00E+00 0,00E+00 0,00E+00 0 0,00E+00 0,00E+00 0,00E+00 0,00E+00
MFR kg 1,14E-01 0,00E+00 7,10E-04 0 0,00E+00 3,57E+01 0,00E+00 0,00E+00
MER kg 2,15E-01 0,00E+00 3,00E+01 0 0,00E+00 5,09E+01 0,00E+00 0,00E+00
EEE MJ 1,44E-01 0,00E+00 2,09E+01 0 0,00E+00 7,82E+01 0,00E+00 0,00E+00
EET MJ 2,17E+00 0,00E+00 3,16E+02 0 0,00E+00 1,18E+03 0,00E+00 0,00E+00
CRU = Components for re-use; MFR = Materials for recycling; MER = Materials for energy recovery; EEE = Exported energy electrical; EET = Exported energy thermal
"Reading example: 9,0 E-03 = 9,0*10-3 = 0,009"
*INA Indicator Not Assessed
Biogenic Carbon Content
Indicator Unit At the factory gate
Biogenic carbon content in product kg C 0,00E+00
Biogenic carbon content in accompanying packaging kg C 1,25E+01
Note: 1 kg biogenic carbon is equivalent to 44/12 kg CO2
9 / 11
Additional requirements
Greenhouse gas emissions from the use of electricity in the manufacturing phase
National production mix from import, low voltage (production of transmission lines, in addition to direct emissions and losses in grid) of applied
electricity for the manufacturing process (A3).
Electricity mix Source Amount Unit
Electricity, Czech Republic (kWh) ecoinvent 3.6 942,91 g CO2-eq/kWh
Dangerous substances
The product contains no substances given by the REACH Candidate list.
Indoor environment
Additional Environmental Information
Additional environmental impact indicators required in NPCR Part A for construction products
Indicator Unit A1-A3 A4 A5 C1 C2 C3 C4 D
GWPIOBC kg CO2 -eq 9,46E+02 4,03E+01 8,07E-01 0 2,17E+00 1,25E+02 4,15E-01 -3,17E+02
GWP-IOBC: Global warming potential calculated according to the principle of instantaneous oxidation. In order to increase the transparency of biogenic carbon​
contribution to climate impact, the indicator GWP-IOBC is required as it declares climate impacts calculated according to the principle of instantaneous oxidation.​
GWP-IOBC is also referred to as GWP-GHG in context to Swedish public procurement legislation.
10 / 11
Bibliography
ISO 14025:2010 Environmental labels and declarations - Type III environmental declarations - Principles and procedures.
ISO 14044:2006 Environmental management - Life cycle assessment - Requirements and guidelines.
EN 15804:2012+A2:2019 Environmental product declaration - Core rules for the product category of construction products.
ecoinvent v3, Allocation, cut-off by classification, Swiss Centre of Life Cycle Inventories.
EN 50693:2019. Product category rules for life cycle assessments of electronic and electrical products and systems. European Committee for
Standardization.
Iversen et al., (2021) eEPD v2021.09 Background information for EPD generator tool system verification, LCA.no Report number: 07.21
Babwah, R., Philis, G. (2024). EPD generator for EPD Italy PCR 010 Insulators, background information for EPD generator application and LCA data,
LCA.no. Report number: 04.24. PCR verification report.
EPD Italy (2020). PCR EPD Italy 007 Part A for electronic and electrical products and systems. EPD Italy. Version 3, issue 20-01-2020 and valid
until 19-01-2025.
EPD Italy (2021). PCR EPD Italy 010 Part B for Insulators EPD Italy. Version 0, issue 16-03-2020 and valid until 15-03-2025.
Program operator and publisher Phone: +47 977 22 020
The Norwegian EPD Foundation e-mail: post@epd-norge.no
Post Box 5250 Majorstuen, 0303 Oslo, Norway web: www.epd-norge.no
Owner of the declaration: Phone:
Maxeta AS e-mail: maxeta@maxeta.no
Amtmand Aallsgate 89, 3716 Skien web:
Author of the Life Cycle Assessment Phone: +47 916 50 916
LCA.no AS e-mail: post@lca.no
Dokka 6A, 1671 Kråkerøy web: www.lca.no
Developer of EPD generator Phone: +47 916 50 916
LCA.no AS e-mail: post@lca.no
Dokka 6A, 1671 Kråkerøy web: www.lca.no
ECO Platform web: www.eco-platform.org
ECO Portal web: ECO Portal
11 / 11
