ver1 2017
ENVIRONMENTAL PRODUCT DECLARATION
-in accordance with ISO 14025, ISO 21930 and EN 15804
Owner of the declaration: Saint-Gobain Finland Oy / ISOVER
Program operator: The Norwegian EPD Foundation
Publisher: The Norwegian EPD Foundation
Declaration number: NEPD-2229-1019-EN
Registration number: NEPD-2229-1019-EN
ECO Platform reference number: -
Issue date: 02.06.2020
Valid to: 02.06.2025
ISOVER CC CRoll Alu1
Saint-Gobain Finland Oy / ISOVER
www.epd-norge.no
www.epd-norge.no
NEPD-2229-1019-EN ISOVER CC CRoll Alu1
General information
Product
ISOVER CC CRoll Alu1
Owner of the declaration
Program operator
Saint-Gobain Finland Oy / ISOVER
The Norwegian EPD Foundation
Post Box 5250 Majorstuen, 0303 Oslo
Contact person: Janne Vainio
Phone: +47 97722020
Phone: +358 10 442 200
E-mail: post@epd-norge.no
E-mail: janne.vainio@saint-gobain.com
Web: www.epd-norge.no
Manufacture
Declaration number
Saint-Gobain Finland Oy / ISOVER
NEPD-2229-1019-EN
Place of production
ECO Platform reference number
Forssa, Finland
Place of usage
This declaration is based on Product Category
Finland, Estonia, Latvia and Lithuania
Rules
CEN Standard EN 15804 serve as core PCR.
Management system
The Product Category Rules, NPCR 012:2018 Part B
DS/EN ISO 9001:2015
for Thermal Insulation products is used in addition to
DS/EN ISO 14001:2015
the core PCR.
Org. No.
Statement of liability
1020917543
The owner of the declaration shall be liable for the
underlying information and evidence.
Issue date
EPD Norway shall not be liable with respect to
manufacturer information, life cycle assessment data 02.06.2020
and evidences.
Valid to
Declared unit 02.06.2025
1 m² with a thermal resistance of 1.0 m²K/W with a
Year of study
thickness of 36 mm.
2018
Functional unit
Comparability
1 m² with a thermal resistance of 1.0 m²K/W with a
EPD of construction products may not be
reference service life of 60 years.
comparable if they do not comply with EN15804 and
seen in a building context.
Verification
Independent verification of calculation data and other
The EPD has been worked out by
environmental information and test of the computer
The EPD has been worked out by the use of the
program was carried out by Martin Erlandsson in
tool GaBi, version 8.7 by Saint-Gobain ISOVER
accordance with ISO14025, 8.1.3 and 8.1.4 + EN 15804
Team by Janne Vainio
Externally
Company-specific data has been verified by
SG central LCA team.
Approved
IVL Swedish Environmental Research Institute
(Independent verifier approved by EPD Norway)
2
NEPD-2229-1019-EN ISOVER CC CRoll Alu1
Product description
Product description and description of use:
This EPD describes the potential environmental impacts of 1 m² of glass wool insulation, ISOVER CC
CRoll Alu1, with a thermal resistance equal to 1.00 m2K/W
The intended use of this EPD is to communicate scientifically based environmental information for
construction products, for the purpose of assessing the environmental performance of buildings.
ISOVER glass wool products are CE-labelled according to EN 14303 (2009) “Thermal Insulation
Products for Building Equipment and Industrial Installations. Factory made mineral wool (MW) Products.
Specification”, and EN 13172 (2012) “Thermal Insulation Products – Evaluation of Conformity”
The production site of Saint-Gobain Finland Oy / ISOVER in Forssa Finland, use a small amount of
natural and abundant raw materials (sand, soda, limestone, feldspar) and a high share of recycled glass
cullets (more than 50 % of external glass cullets). This material is converted by using fusion and
fiberizing techniques to produce glass wool. The products obtained come in the form of "mineral wool
slabs, rolls or lamellas" consisting of a soft, airy structure.
On Earth, naturally, the best insulator is dry immobile air at 10 °C: its thermal conductivity factor,
expressed in λ, is 0.025 W/(mK) (watts per meter Kelvin degree). The thermal conductivity of mineral
wool is close to immobile air as its lambda varies from 0.030 W/(mK) for the most efficient, to 0.040 W/
(mK) to the least efficient.
With its entangled structure, glass wool is a porous material that traps the air, making it one of the best
insulating materials. The porous and elastic structure of the wool also absorbs airborne noise, impact
noise and offers acoustic correction inside premises.
Glass wool containing incombustible materials does not react to fire.
Glass wool insulation is used in buildings as well as industrial facilities. It ensures a high level of comfort
and minimizes carbon dioxide (CO ) emissions by preventing heat loss through roofs, walls, floors, pipes
2
and boilers. It reduces noise and protects homes and industrial facilities against fire.
Correctly installed glass wool products and solutions do not require maintenance and last throughout
the lifetime of the building (which is set at 60 years as a default value in the model), or as long as the
insulated building component is a part of the building.
3
NEPD-2229-1019-EN ISOVER CC CRoll Alu1
Technical data/physical characteristics (for a thickness of 36 mm):
The thermal resistance of the product: 1.00 m²K/W
The thermal conductivity of the product: 0.036 W/(mK)
Product density: 20 – 30 mm 30,0 kg/m3
50 – 100 mm 22,0 kg/m3
Description of the main product components and/or materials:
Mineral wool 90-95 % (REACH registration number 01-2119472313-44-0039)
Binder 0-10 %
PARAMETER VALUE
Quantity of mineral wool 1080 g
Thickness of mineral wool 36 mm
Surfacing Aluminum 98,5 g/m2
Polyethylene 22,7 g/m2
Packaging for the transportation and distribution Paper 32,9 g/m2
Wood 103,4 g/m2
Product used for the Installation None
LCA calculation information
FUNTIONAL UNIT
Providing a thermal insulation on 1 m² with a thermal
resistance of equals 1 m2K/W a thickness of 36 mm
SYSTEM BOUNDARIES Cradle to Grave. Mandatory stages: A1-3, A4-5, B1- 7,
C1-4
REFERENCE SERVICE LIFE (RSL) 60 years
CUT-OFF RULES See below
ALLOCATIONS
See below
ELECTRICITY USED FOR THE
Renewable electricity mix (reference year 2018)
MANUFACTORING PROCESS
GEOGRAPHICAL COVERAGE AND TIME
PERIOD Finland, 2018
Cut-off criteria
The cut-off criterion used in Saint-Gobain EPD will be the mass criterion with the following details:
- Taking into account all input and output flows in a unit process i.e. taking into account the value of all
flows in the unit process and the corresponding LCI whenever available
- No simplification of the LCI by additional exclusions of material flows
Data collected at the manufacturing site was used. The inventory process in this LCA includes all data related
4
NEPD-2229-1019-EN ISOVER CC CRoll Alu1
to raw material, packaging material and consumable items, and the associated transport to the manufacturing
site. Process energy and water use, direct production waste and emissions to air and water are included.
Scenarios have been developed to account for downstream processes such as demolition and waste treatment
in accordance with the requirements of EN 15804:2012+A1:2013
All inputs and outputs to the manufacturing plants have been included and made transparent. All assumptions
regarding the materials and water balances have also been included.
All hazardous and toxic materials and substances are considered in the inventory even though they are below
the cut off criteria
There are excluded processes in the inventory:
- Flows related to human activities such as employee transport and administration activity.
Allocation
Allocation criteria are based on mass.
The allocation of all the air emissions, wastes and energy usage are based on mass (kg). The reason we can
use a mass basis is because we use the exact same manufacturing process shown for every product. We only
produce glass mineral wool in the Hyvinkää and Forssa sites using the same process and therefore all the
factors can be allocated by a mass basis. The amount of binder varies for different products and is accounted
for as well as if different surface layers are used.
A mass balance was conducted for the 2018 production year to ensure that we have not excluded any materials,
emissions and hence potential environmental impacts. Regarding the mass balance, all the raw materials and
corresponding production goods and wastes generated were taken into account.
5
NEPD-2229-1019-EN ISOVER CC CRoll Alu1
Flow diagram of the Life Cycle
A1-A3 Product stage A4-A5 Construction process
Sand and other
A1-A3 Production
minerals Additional
Diesel
Wood pallet and production due to
Cullet Polyethylene losses 2%
packaging
Binder
A1 – A3 Production A4 A5
Transport Installation
Internal
Natural Gas recycling
Electricity Primary product
Diesel
Evaporation
Water
Air
Waste Emission
Losses: 2%
Packaging waste
External
PCR for Insulation products has 5% waste as default,
Landfill Recycling
see detailed explanation at page 8
B1-B7 Use C1-C4 End-of-life
Diesel
B1-B5 use B6-B7 operation C1 de- C2 transport C3 waste C4 disposal
of the building construction, to waste processing
demolition processing for reuse,
recovery
and/or
recycling
Waste (glass
wool product):
100%
Landfilled
6
NEPD-2229-1019-EN ISOVER CC CRoll Alu1
System boundaries (X = included, MND = Module not declared)
Beyond the
Construction
Product stage Use stage End of life stage system
installation stage
boundaries
7
slairetam
waR
tropsnarT
gnirutcafunaM
tropsnarT
noitallatsni
noitcurtsnoC
egats esU
ecnanetniaM
riapeR
tnemecalpeR tnemhsibrufeR
esu
ygrene
lanoitarepO
esu
retaw
lanoitarepO
noitcurtsnoc-eD
noitilomed tropsnarT
gnissecorp
etsaW
lasopsiD
-yrevoceR-esueR laitnetop-gnilcyceR
A1 A2 A3 A4 A5 B1 B2 B3 B4 B5 B6 B7 C1 C2 C3 C4 D
X X X X X X X X X X X X X X X X MND
Product stage, A1- A3
Description of the stage:
The product stage of the mineral wool products is subdivided into 3 modules A1, A2 and A3
respectively “Raw material supply”, “transport” and “manufacturing”.
The aggregation of the modules A1, A2 and A3 is a possibility considered by the EN 15804
standard. This rule is applied in this EPD.
A1, Raw material supply
This module takes into account the extraction and processing of all raw materials and energy
which occur upstream to the studied manufacturing process.
Specifically, the raw material supply covers production of binder components and sourcing
(quarry) of raw materials for fiber production, e.g. sand and borax for glass wool. Besides these
raw materials, glass cullet is also used as input.
About cullet: The main raw material for the production of glass insulation material is cullets
or/and sand. Only specific cleaning activities and transport is included for the cullets – and thus
not the impacts from the full life cycle of glass. The reason is that cullets are considered a waste
product and not initially produced for the purpose of glass wool insulation production.
The only activities included are:
- Magnetic separation of metallic piece
- Separation of other piece-crushing of glass (<20 mm)
- Separation of bottle cap crushing (<2 mm) sieving
- Transport
A2, Transport to the manufacturer
The raw materials are transported to the manufacturing site. In our case, the modeling include:
road and boat transportations (specific values) of each raw material.
A3, Manufacturing
This module covers glass wool fabrication, including melting and fiberizing (see process flow
diagram). In addition, the production of packaging material is taking into account at this stage.
NEPD-2229-1019-EN ISOVER CC CRoll Alu1
Manufacturing process flow diagram
Construction process stage, A4- A5
Description of the stage:
The construction process is divided into 2 modules: A4, transport to the building site and A5,
installation in the building.
Description of scenarios and additional technical information:
A4, Transport to the building site:
This module includes transport from the production gate to the building site.
Transport is calculated on the basis of a scenario with the parameters described in the following
table.
PARAMETER VALUE
Fuel type and consumption of vehicle or vehicle
Average truck trailer with a 27t payload, diesel
type used for transport e.g. long distance truck,
consumption 31,6 liters for 100 km
boat, etc.
Distance 150 km
100 % of the capacity in volume
Capacity utilisation (including empty returns)
30 % of empty returns
Bulk density of transported products 65 kg/m3 (compressed density*)
Volume capacity utilisation factor 1.00
*Isover products presents a compression factor between 1 and 4. For an average volume of the truck of 90 m³ and the
m2 of product specified in the prices.
8
NEPD-2229-1019-EN ISOVER CC CRoll Alu1
A5, Installation into the building:
This module includes:
- Wastage of products: 2 %. These losses are landfilled (landfill model for glass, see
chapter End-of-life)
- Additional production processes to compensate for the loss
- Processing of packaging wastes: they are 100 % collected and modeled as recovered
matter.
This module does not include:
- Energy for installation of the insulation, as the installation is done manually, and do not
require energy
PARAMETER VALUE
Wastage of materials on the building site before
waste processing, generated by the product’s 2 %*
installation (specified by type)
Packaging wastes are 100 % collected and modeled
Output materials (specified by type) as results of as recovered matter
waste processing at the building site e.g. of
collection for recycling, for energy recovering, Following a conservative methodology mineral wool
disposal (specified by route) losses are considered to be landfilled, while they are
100% recyclable and/or reusable.
Use stage (excluding potential savings), B1- B7
Description of the stage:
The use stage is divided into the following modules:
- B1: Use
- B2: Maintenance
- B3: Repair
- B4: Replacement
- B5: Refurbishment
- B6: Operational energy use
- B7: Operational water use
Description of scenarios and additional technical information:
Once installation is complete, no actions or technical operations are required during the use stages until
the end-of-life stage. Therefore glass wool insulation products have no impact (excluding potential
energy savings) on this stage.
End-of-life stage, C1- C4
Description of the stage:
The stage includes the following different modules of end-of-life:
C1, De-construction, demolition
The de-construction and/or dismantling of insulation products are part of the demolition of the
entire building, and are assumed to be made manually. In our case, the environmental impact is
assumed to be very small and can be neglected.
C2, Transport to waste processing
Transport is included and calculated on the basis of a scenario with the parameters described in
the End-of-life table below.
C3, Waste processing for reuse, recovery and/or recycling
Today the product is considered to be landfilled without reuse, recovery or recycling.
C4, Disposal
9
NEPD-2229-1019-EN ISOVER CC CRoll Alu1
The glass wool is assumed to be 100% landfilled.
Description of scenarios and additional technical information: See below
PARAMETER DESCRIPTION
The entire insulation product (wool) is collected with
mixed construction waste.
Collection process specified by type
1,080 kg of glass wool (collected with mixed
construction waste)
Recovery system specified by type No re-use, recycling or energy recovery
The entire insulation product (wool) is landfilled.
Disposal specified by type
1,080 kg of glass wool are landfilled
Average truck trailer with a 24t payload, diesel
consumption 38 liters for 100 km.
Assumptions for scenario development (e.g.
25 km (default distance from the building site to
transportation)
landfill).
Min. 30% empty returns
Reuse/recovery/recycling potential, D
Module D is not included in the EPD.
LCA results
LCA model, aggregation of data and potential environmental impact are calculated from the GaBi
software 8.7 and CML impact method has been used, together with thinkstep 8.7 (2018) and ecoinvent
V3.1 (2014) databases to obtain the inventory of generic data. Biogenic carbon is not reported in the
context of GWP.
Raw materials and energy consumption, as well as transport distances have been taken directly from
the manufacturing plant of Saint-Gobain Finland Oy / ISOVER in Forssa (Production data according
2018).
Resume of the LCA results detailed on the following tables.
10
NEPD-2229-1019-EN ISOVER CC CRoll Alu1
ENVIRONMENTAL IMPACTS
Product Construction
Use stage End-of-life stage
stage process stage
Parameters
11
3A
/
2A
/
1A
tropsnarT
4A
noitallatsnI
5A
esU
1B
ecnanetniaM
2B
riapeR
3B
4B
tnemecalpeR
5B
tnemhsibrufeR lanoitarepO
6B
esu
ygrene
lanoitarepO
7B
esu
retaw 1C
/ noitcurtsnoceD noitilomed tropsnarT
2C
etsaW
3C
gnissecorp lasopsiD
4C
,yrevocer
,esueR
D
gnilcycer
1,45E+00 8,38E-02 3,28E-02 0 0 0 0 0 0 0 0,00E+00 7,07E-03 0 1,32E-01 MND
Global Warming Potential
(GWP) - kg CO equiv/FU
2 The global warming potential of a gas refers to the total contribution to global warming resulting from the emission
of one unit of that gas relative to one unit of the reference gas, carbon dioxide, which is assigned a value of 1.
4,45E-08 1,28E-17 8,91E-10 0 0 0 0 0 0 0 0,00E+00 6,13E-15 0 1,43E-16 MND
Ozone Depletion (ODP)
kg CFC-11 equiv/FU Destruction of the stratospheric ozone layer which shields the earth from ultraviolet radiation harmful to life.
This destruction of ozone is caused by the breakdown of certain chlorine and/or bromine containing compounds (chlorofluorocarbons or halons),
which break down when they reach the stratosphere and then catalytically destroy ozone molecules.
1,29E-02 3,80E-04 2,66E-04 0 0 0 0 0 0 0 0,00E+00 2,96E-05 0 1,46E-04 MND
Acidification potential (AP)
kg SO equiv/FU
2 Acid depositions have negative impacts on natural ecosystems and the man-made environment incl, buildings.
The main sources for emissions of acidifying substances are agriculture and fossil fuel combustion used for electricity production, heating and transport.
Eutrophication potential (EP) 3,75E-03 9,40E-05 7,92E-05 0 0 0 0 0 0 0 0,00E+00 7,18E-06 0 1,46E-04 MND
kg (PO)3- equiv/FU
4
Excessive enrichment of waters and continental surfaces with nutrients, and the associated adverse biological effects.
Photochemical ozone 9,28E-04 1,39E-05 1,97E-05 0 0 0 0 0 0 0 0,00E+00 1,10E-06 0 4,52E-05 MND
creation (POPC)
kg Ethene equiv/FU Chemical reactions brought about by the light energy of the sun.
The reaction of nitrogen oxides with hydrocarbons in the presence of sunlight to form ozone is an example of a photochemical reaction.
Abiotic depletion potential for
non-fossil resources (ADP- 1,14E-04 1,11E-09 2,29E-06 0 0 0 0 0 0 0 0,00E+00 9,55E-11 0 8,28E-09 MND
elements) - kg Sb equiv/FU
Abiotic depletion potential for
2,14E+01 1,16E+00 4,51E-01 0 0 0 0 0 0 0 0,00E+00 9,84E-02 0 4,62E-01 MND
fossil resources (ADP-fossil
fuels) - MJ/FU
Consumption of non-renewable resources, thereby lowering their availability for future generations.
NEPD-2229-1019-EN ISOVER CC CRoll Alu1
RESOURCE USE
Product Construction
Use stage End-of-life stage
stage process stage
Parameters
12
3A
/
2A
/
1A
tropsnarT
4A
noitallatsnI
5A
esU
1B
ecnanetniaM
2B
riapeR
3B
4B
tnemecalpeR
5B
tnemhsibrufeR lanoitarepO
6B
esu
ygrene
lanoitarepO
7B
esu
retaw 1C
/ noitcurtsnoceD noitilomed tropsnarT
2C
etsaW
3C
gnissecorp lasopsiD
4C
,yrevocer
,esueR
D
gnilcycer
Use of renewable primary
energy excluding renewable
2,64E+01 2,7E-02 5,3E-01 0 0 0 0 0 0 0 0 2,5E-03 0 4,5E-02 MND
primary energy resources used
as raw materials - MJ/FU
Use of renewable primary
energy used as raw materials 2,34E+00 - 4,7E-02 - - - - - - - - - - - MND
MJ/FU
Total use of renewable primary
energy resources (primary energy
2,87E+01 2,7E-02 5,8E-01 0 0 0 0 0 0 0 0 2,5E-03 0 4,5E-02 MND
and primary energy resources used
as raw materials) - MJ/FU
Use of non-renewable primary
energy excluding non-renewable
2,42E+01 1,2E+00 5,1E-01 0 0 0 0 0 0 0 0 9,9E-02 0 4,8E-01 MND
primary energy resources used
as raw materials - MJ/FU
Use of non-renewable primary
energy used as raw materials - 3,46E+00 - 6,9E-02 - - - - - - - - - - - MND
MJ/FU
Total use of non-renewable primary
energy resources (primary energy
2,76E+01 1,2E+00 5,8E-01 0 0 0 0 0 0 0 0 9,9E-02 0 4,8E-01 MND
and primary energy resources used
as raw materials) - MJ/FU
Use of secondary material
8,73E-01 0 1,8E-02 0 0 0 0 0 0 0 0 0 0 0 MND
kg/FU
Use of renewable secondary
0 0 0 0 0 0 0 0 0 0 0 0 0 0 MND
fuels - MJ/FU
Use of non-renewable
0 0 0 0 0 0 0 0 0 0 0 0 0 0 MND
secondary fuels - MJ/FU
Use of net fresh water - m3/FU 2,36E-02 8,9E-06 4,7E-04 0 0 0 0 0 0 0 0 8,2E-07 0 7,3E-05 MND
NEPD-2229-1019-EN ISOVER CC CRoll Alu1
WASTE CATEGORIES
Product Construction
Use stage End-of-life stage
stage process stage
Parameters
13
3A
/
2A
/
1A
tropsnarT
4A
noitallatsnI
5A
esU
1B
ecnanetniaM
2B
riapeR
3B
4B
tnemecalpeR
5B
tnemhsibrufeR lanoitarepO
6B
esu
ygrene
lanoitarepO
7B
esu
retaw 1C
/ noitcurtsnoceD noitilomed tropsnarT
2C
etsaW
3C
gnissecorp lasopsiD
4C
,yrevocer
,esueR
D
gnilcycer
Hazardous waste disposed
7,33E-08 4,18E-09 1,61E-09 0 0 0 0 0 0 0 0,00E+00 3,54E-10 0 4,68E-09 MND
kg/FU
Non-hazardous waste disposed
kg/FU
2,08E-01 1,41E-05 3,04E-02 0 0 0 0 0 0 0 0,00E+00 1,31E-06 0 1,19E+00 MND
Radioactive waste disposed
5,84E-04 1,36E-06 1,18E-05 0 0 0 0 0 0 0 0,00E+00 1,15E-07 0 6,34E-06 MND
kg/FU
NEPD-2229-1019-EN ISOVER CC CRoll Alu1
OUTPUT FLOWS
Product Construction
Use stage End-of-life stage
stage process stage
Parameters
14
3A
/
2A
/
1A
tropsnarT
4A
noitallatsnI
5A
esU
1B
ecnanetniaM
2B
riapeR
3B
4B
tnemecalpeR
5B
tnemhsibrufeR lanoitarepO
6B
esu
ygrene
lanoitarepO
7B
esu
retaw 1C
/ noitcurtsnoceD noitilomed tropsnarT
2C
etsaW
3C
gnissecorp lasopsiD
4C
,yrevocer
,esueR
D
gnilcycer
Components for re-use
0 0 0 0 0 0 0 0 0 0 0 0 0 0 MND
kg/FU
Materials for recycling
kg/FU
1,27E-02 0 1,28E-01 0 0 0 0 0 0 0 0 0 0 0 MND
Materials for energy recovery
0 0 0 0 0 0 0 0 0 0 0 0 0 0 MND
kg/FU
Exported energy
0 0 0 0 0 0 0 0 0 0 0 0 0 0 MND
MJ/FU
NEPD-2229-1019-EN ISOVER CC CRoll Alu1
Product Transport Installation Use End-of-life
(A1-A3) (A4) (A5) (B) (C) Total
Environmental
impacts of the
product
Global warming 2,00
1,45
1,50
1,71
1,00
0,50 0,08 0,03 0,00 0,14
0,00
Non-renewable resources 30,00
consumption [1] 21,40
20,00 23,57
10,00
1,16 0,45 0,00 0,56
0,00
Energy consumption [2] 60,00 56,30
40,00 59,27
20,00
1,20 1,15 0,00 0,62
0,00
Water consumption [3] 0,03
0,0236
0,02 0,02
0,01
0,0000 0,0005 0,0000 0,0001
0,00
Waste production [4] 1,50
1,19
1,00 1,43
0,50 0,21
0,00 0,03 0,00
0,00
[1] This indicator corresponds to the abiotic depletion potential of fossil resources.
[2] This indicator corresponds to the total use of primary energy.
[3] This indicator corresponds to the use of net fresh water.
[4] This indicator corresponds to the sum of hazardous, non-hazardous and radioactive waste disposed.
15
UF/viuqe2OC
gk
UF/JM
UF/JM
UF/3m
UF/gk
LCA interpretation
kg CO equiv/FU 2
MJ/FU
MJ/FU
m3/FU
kg/FU
NEPD-2229-1019-EN ISOVER CC CRoll Alu1
ADDITIONAL INFORMATION
Influence of particular thicknesses
All the results in the table of this EPD refer to ISOVER CC CRoll Alu1 with a thickness of 36 mm for a functional
unit of 1 m² with a thermal resistance equals to 1.00 m2K/W
This EPD of ISOVER CC CRoll Alu1 includes a range of thicknesses between 20 mm and 100 mm. For every
thickness, use a multiplication factor in order to obtain the environmental performance of every thickness. In order
to calculate the multiplication factors, a reference unit has been selected (value of R= 1.00 m2K/W for 36 mm).
The various multiplication factors are obtained by making the LCA calculations for all thicknesses, including
packaging.
In the table below the multiplication factors are shown for products and specific thickness of the product family. In
order to obtain the environmental performance associated with every specific product and thickness, the results
expressed in this EPD must be multiplied by its corresponding multiplication factor. Such factor is based on GWP
indicator and should be used as a proxy for the rest of indicator showed in this EPD. If there is a need for
environmental performance for a thickness not presented in the table below, please use a thickness just above it.
PRODUCT THICKNESS THERMAL
MULTIPLICATION FACTOR
(mm) RESISTANCE
36 1.00 1.00
20 0.56 0.67
30 0.83 0.84
50 1.39 0.94
80 2.22 1.32
100 2.78 1.60
Influence of transportation to others countries
The results of stage A4 (transportation of product) in the table of this EPD refer to transportation in Finland.
This product is also delivered to the countries in the table below. In order to adapt the impact of transportation in
the A4 column, figures from the current EPD shall be multiply by the multiplication factors below.
Country Average distance MULTIPLICATION FACTOR
Finland 150 (Truck) 1,00
Estonia 200 (Truck 110 km, boat 90 km) 0,98
Latvia 510 (Truck 420 km, boat 90 km) 1,12
Lithuania 800 (Truck 710 km, boat 90 km) 1,24
16
NEPD-2229-1019-EN ISOVER CC CRoll Alu1
Additional Norwegian requirements
Greenhouse gas emissions from the use of electricity in the manufacturing phase
The LCA calculation has been made taking into account the fact that during the manufacturing process it is used
100% renewable electricity. This 100% renewable electricity bought is evidenced by Guarantee of Origin certificates
(GOs) from LOS, valid for the period chosen in the calculation (2018).
TYPE OF INFORMATION DESCRIPTION
Location Representative of average production in Finland
Split of energy sources in Finland
Geographical representativeness description -Hydro: 54%
-Biomass: 46%
Reference year 2018
Type of data set Cradle to gate from Thinkstep
Gabi database from International Energy Agency -2013
Source
Guarantee of Origin certificates (GOs) - 2018
The dataset used to model the renewable electricity mix used for these calculations come from thinkstep database.
DATA SOURCE AMOUNT UNIT
thinkstep (2018) 0.05 kg CO2 eq /KWh
Dangerous substances
The product contains no substances given by the REACH Candidate list (of 15.01.2018) or the Norwegian priority
list. (REACH registration number 01-2119472313-44-0039)
Carbon footprint
Carbon footprint has not been worked out for the product
17
NEPD-2229-1019-EN ISOVER CC CRoll Alu1
Bibliography
- Product Category Rules: NPCR 012:2018 Part B for Thermal insulation products
- Environmental labels and declarations - Type III environmental declarations -Principles and procedures
(ISO 14025:2006)
- Environmental management - Life cycle assessment – Requirements and guidelines (ISO 14044:2006)
- Sustainability of construction works - Environmental product declaration - Core rules for the product
category of construction products (EN 15804:2012)
- Ecoinvent database V3.1 (2014)
- Gabi database (2018)
- SS-EN 13172:2012 Thermal Insulation Products – Evaluation of conformity
- SS- EN 14303 “Thermal insulation products for building equipment and industrial installations. Factory made
mineral wool (MW) products. Specification
- LCA report, Information for the Environmental Product Declaration of Isover product. Saint-Gobain Finland
Oy/ Isover, June 2019
Program operator and publisher Phone: +47 97722020
The Norwegian EPD Foundation E-mail: post@epd-norge.no
Post Box 5250 Majorstuen, 0303 Oslo
Web: www.epd-norge.no
Norway
Phone:
Owner of the declaration +358 10 442 200
E-mail:
Saint-Gobain Finland Oy / ISOVER janne.vainio@saint-gobain.com
P.O. Box 70, FI-00381 Helsinki Finland www.isover.fi
Web:
Author of the Life Cycle Assessment
+33 1 47 62 42 65
Patricia Jimenez Diaz Phone:
patricia.jimenezdiaz@saint-
Saint-Gobain, Central Marketing & E-mail:
gobain.com
Development,
18
NEPD-2229-1019-EN ISOVER CC CRoll Alu1
