ENVIRONMENTAL PRODUCT DECLARATION
ISO 14025, ISO 21930 and EN 15804
Owner of the declaration: Paroc Group Oy
Program operator: The Norwegian EPD Foundation
Publisher: The Norwegian EPD Foundation
Declaration number: NEPD-2742-1440-EN
Registration number: NEPD-2742-1440-EN
ECO Platform reference number: -
Issue date: 29.03.2021
Valid to: 29.03.2026
PAROC Stone Wool Thermal Insulation (Ultra)
PAROC Building Insulation
Paroc Group Oy
Owner of the declaration
1/11
NEPD-2742-1440-EN PAROC Stone Wool Thermal Insulation (Ultra)
Product
Product: Owner of the declaration:
PAROC Stone Wool Thermal Insulation (Ultra) Paroc Group Oy
Contact person: Emelia Samuelsson
Program operator: Phone +46 (0) 500 46 90 05
The Norwegian EPD Foundation E-mail: emelia.samuelsson@owenscorning.com
P.O. Box 5250 Majorstuen, N – 0303 Oslo, Norway
Phone: +47 23 08 80 00 Manufacturer:
E-mail: post@epd-norge.no Paroc Group Oy
FI-00181, Helsinki
Declaration number: Finland
NEPD-2742-1440-EN
ECO Platform reference number: Place of production:
<From EPD-Norge> Vilnius, Lithuania
This declaration is based on Product Category
Rules: Management system:
CEN Standard EN 15804 serves as core PCR ISO 14001 and ISO 9001
NPCR 012:2018 version 2. Part B for Thermal
insulation products Organisation no:
LCA of PAROC stone wool produced at Lithuanian 23025016
plant.
Issue date:
Statement of liability: 29.03.2021
The owner of the declaration shall be liable for the
underlying information and evidence. Valid to:
EPD Norway shall not be liable with respect to 29.03.2026
manufacturer information, life cycle assessment data
and evidences. Year of study:
2018
Declared unit:
1 m² of stone wool with a thermal resistance (R) of 1 Comparability:
Km2/W. 1 m2 PAROC Ultra at R=1 is at a weight of
EPD of construction products may not be comparable
1,13 kg.
if they not comply with EN 15804 and seen in a
building context.
Declared unit with option:
-
Functional unit:
1 m² of stone wool with thermal resistance (R) of 1
m2K/W with a reference service life of minimum 60
years. Impact exclude any lamination.
The EPD has been worked out by:
Emelia Samuelsson, Paroc AB
Verification:
The CEN Norm EN 15804 serves as the core PCR.
Independent verification of the declaration and data,
according to ISO14025:2010
☐internal ☒external Approved
Martin Erlandsson, IVL
(Independent verifier approved by EPD Norway)
2/11
NEPD-2742-1440-EN PAROC Stone Wool Thermal Insulation (Ultra)
Product
Product description: Product content:
Stone wool is made from volcanic rock, typically basalt
Materials %
or dolomite, and an increasing proportion of recycled
material. Stone wool is a wide spread building material
Mineral Wool 96-99%
which is mainly used for thermal insulation. Behind the
product there is an 80-year history of stone wool
Binder (phenol-formaldehyde-urea- 0-6%
production knowhow backed with technical insulation
copolymer)
expertise and innovation.
Dustbinding (mineral oil) 0,1-0,5%
Market:
Technical data:
Mainly Lithuania, Latvia, Estonia, Poland, Russia,
Ukraine, Belarus.
Name Value Unit
Thermal conductivity 0,035 W/(mK)
Reference service life: EN 12939 and
EN 12667
The reference service lifetime of PAROC products is
equal to the reference service life of the building. For
Thickness Class T2
the purpose of this EPD the reference service life is
EN 823
considered to be minimum 60 years, which is usually
EN 12431
the assumption about the lifetime of the building where
this is installed.
Fire Class A1
EN 13501-1:2007+
A1:2009/
Length and width EN 822 L± 2 %
W ± 1,5
Compressive Strength NDP
EN 827
Dimension Stability at DS(70,-)
spec. temperature and
humidity
EN 1604
Tensile strength NDP
perpendicular to faces
/EN1607/
Water vapour diffusion 1
resistance factor
/EN12086/
Point Load /EN12430/ NDP
3/11
NEPD-2742-1440-EN PAROC Stone Wool Thermal Insulation (Ultra)
LLCCAA:: CCaallccuullaattiioonn RRuulleess
Functional unit: System boundary:
1 m² stone wool with a thermal resistance (R) of 1 Table below identifies the modules included in this
Km2W-1. study.
The calculation of the weight per square meter is done According to EN 15804 any declared benefits and
as follows: loads from net flows leaching the product system not
allocated as co-products and have passed the end-of-
m2-weight = density [kg/m3] x insulation thickness [m] waste state shall be included in the module D. Module
(in order to meet a specific thermal resistance) = D includes reuse, recovery and/or recycling potentials.
m2-weight insulation = density [kg/m3[ x R [m2K/W] x
λ [W/m K] = [kg/m2]. The production stage (A1-A3) covers the following
steps:
The specific product, referred to in the declared unit,
is 1 m2 (32,4 kg/m3) of PAROC Ultra, 100 mm • Raw materials production (e.g. dolomite,
thickness from the product group of flexible slabs and diabase)
mats. • Components production (e.g. resin)
• Transports of raw materials and pre-products
Data quality:
to manufacturing plants
The stone wool production data is site specific from • Production of packaging materials
PAROC plant in Vilnius, Lithuania. Foreground data • Waste management, water treatment, end-of-
refer to the year 2018.
life of residues
For life cycle modeling the GaBi 9 Software System for
With the exception of Modules A1 to A3 (describing
Life Cycle Assessment, developed by Sphera
the manufacturing of stone wool) all other modules are
Solutions, Inc. (formerly known as thinkstep AG), is
calculated on the basis of assumptions or scenarios.
used (/GaBi 9 2020/). All relevant background
datasets are taken from the GaBi 9 software database. The following scenarios were considered in this study:
To ensure comparability of results in the LCA, the
• Modules A4: The average distance to building
basic data of GaBi database were used for energy,
site is 450 km.
transportation and auxiliary materials.
• Modules A5: Packaging waste processing,
The datasets are complete and conform to the system waste generated at the installation is assumed
boundaries and the criteria for the exclusion of inputs to be 0 %.
and outputs. • Modules C2-C4: Similar to installation
scenario with similar kind of waste. In C2 a
Background data refer to the years 2018 until 2021
transport to waste treatment distance 50 km is
(/GaBi 9 2020/) with a country specific scope as far as
assumed.
available, e.g. for raw material extraction and
• Module D: Credits from waste treatment
production, transportation, fuels and energy supply.
(recycling and incineration with energy
All relevant processes (foreground and background) recovery) of product parts after use and from
have been considered when modelling stone wool installation losses.
production. The process data and the used
Cut-off criteria:
background data are consistent. The data quality can
be qualified as good. All major raw materials and all the essential energy is
included. The production process for raw materials
Allocation:
and energy flows that are included with very small
The allocation is made in accordance with the amounts (<1%) are not included. This cut-off rule does
provisions of EN 15804. not apply for hazardous materials and substances.
Incoming energy, water and waste production in- The declared unit is 1 m2 stone wool without any
house is allocated equally among all products through lamination.
mass allocation. Effects of primary production of
recycled materials allocated to the main product in
which the material was used. The recycling process
and transportation of the material is allocated to this
analysis.
4/11
NEPD-2742-1440-EN PAROC Stone Wool Thermal Insulation (Ultra)
LCA: System Boundaries
5/11
NEPD-2742-1440-EN PAROC Stone Wool Thermal Insulation (Ultra)
LLCCAA:: SScceennaarriiooss aanndd AAddddiittiioonnaall TTeecchhnniiccaall IInnffoorrmmaattiioonn
The following information describe the scenarios in the different modules of the EPD.
Transports to the customer are calculated on the basis of a scenario with an average truck trailer with a 27 t payload.
For the final stone wool product, a loading ratio of 30 % of weight capacity has been set. The average transport
distance to the customer is assumed to be 450 km as a basis for this study.
Transport to the Building Site (A4)
Type Capacity utilisation Type of vehicle Distance km Energy use per km Total energy use
(incl. return)
%
Truck 100% (30% weight Truck fleet 450 0,9 liter 418,5 liter
capacity) (0,46 liter/m3 stone wool)
Installation in the Building (A5)
Parameter Parameter expressed by functional unit
Auxiliary materials for the installation Not applicable
Consumption of other resources Not applicable
Quantitative description of the type of energy and consumption Not applicable
rate during the installation process
Wastes at the construction site generated from the installation Installation waste is assumed to be 0% since all
of the product material can be used within the building
Material outputs as a result from waste management processes Waste management process for packaging
at the installation site. For example, compilation for recycling, materials
for energy recovery and final disposal
Emissions to air, soil and water Not applicable
End of Life (C1, C2, C3, C4)
Parameter Parameter expressed by functional unit
Compilation processes district Not applicable
Recycling systems Not applicable
Final disposal Landfilling
Benefits/loads Beyond the System Boundary (D)
Materials that create a benefit in Module D are packaging ma terials. Benefits from the packaging waste treatment
are considered in module D. Energy products of incineration (e.g. steam, electricity, metals) are credited using
the European production averages (e.g. European grid mix f or power). Credits are reported in module D.
6/11
NEPD-2742-1440-EN PAROC Stone Wool Thermal Insulation (Ultra)
LLCCAA:: RReessuullttss
Life Cycle Impact Assessment results represent the environmental impacts for the life cycle of stone wool from
cradle to grave.
The goal is to address all necessary parameters according to EN 15804 for creating EPDs. In a first step the results
are calculated based on 1 kg stone wool representing the PAROC average. After that the data is scaled according
to the provided density and lambda and fixed to the mass required for one square meter product with the respective
R value = 1.
The PAROC Building Insulation products are clustered according to their application into different product groups.
Scaling factors are included in the EPD indicating the factor which to multiply with the indicators in order to get the
environmental burden on product level described. The scaling factors solely refer to the stone wool used in these
products, and thus do not include the different facings. Due to this fact, the variation is less than 10% by reason of
the density, lambda and binder. E.g. Solid (thickness 42-200); 0,98 (scaling factor) multiplied with 1,26 (GWP value
for A1-A3) equals 1,23 kg CO 2—eq per m2.
Product groups
Flexible Slabs & Mats
Special Applications
Facades
Metal Panel Core
Roofs
7/11
NEPD-2742-1440-EN PAROC Stone Wool Thermal Insulation (Ultra)
LCA: Results
Environmental Impact: 1m2 PAROC Ultra (per 1,13 kg)
Parameter Unit A1-A3 A4 A5 C2 C4 D
GWP-TOT* [kg CO -eq] 1,26* 0,0528 0,0964 0,00382 0,0155 -0,0444
2 .
ODP [kg CFC11-eq.] 8,33E- 8,58E-018 1,99E-017 6,22E-019 8,5E-017 -6,09E-016
009
AP [kg SO -eq.] 0,0027 0,000141 1,15E-005 9,33E-006 9,91E-005 -5,51E-005
2
EP [kg PO 3—eq.] 0,000552 3,51E-005 2,49E-006 2,3E-006 1,12E-005 -6,91E-006
4
POCP [kg ethene-eq.] 0,000172 -5,23E-005 9,19E-007 -3,34E-006 7,45E-006 -5,08E-006
ADPM [kg Sb-eq.] 1,79E- 4,34E-009 1,08E-009 3,14E-010 5,96E-009 -8,12E-009
007
ADPE [MJ] 10,8 0,712 0,0212 0,0515 0,219 -0,631
GWP-TOT Global warming potential including emission and uptake of biogenic CO ; ODP Depletion potential of
2
the stratospheric ozone layer; POCP Formation potential of tropospheric photochemical oxidants; AP
Acidification potential of land and water; EP Eutrophication potential; ADPM Abiotic depletion potential for non-
fossil resources; ADPE Abiotic depletion potential for fossil resources.
*A1-3: including 0,0666 kg CO2-eq. uptake of biogenic carbon dioxi de included in product (0 kg CO2-eq.) and packaging
(0,0666 kgCO2-eq.).
Resource Use: 1 m2 PAROC Ultra (per 1,13 kg)
Parameter Unit A 1-3 A4 A5 C2 C4 D
RPEE [MJ] 1,22 - - - - -
RPEM [MJ] 0,717 - - - - -
TPE [MJ] 1,94 0,0401 0,00456 0,0029 0,0296 -0,162
NRPE [MJ] 9,17 - - - - -
NRPM [MJ] 2,5 - - - - -
TRPE [MJ] 11,7 0,714 0,0244 0,0517 0,226 -0,77
SM [kg] 0 0 0 0 0 0
RSF [MJ] 0 0 0 0 0 0
NRSF [MJ] 0 0 0 0 0 0
W [m3] 0,00271 4,64E-005 0,000287 3,36E-006 5,69E-005 -0,000188
RPEE Renewable primary energy resources used as energy carrier; RPEM Renewable primary energy resources
used as raw materials; TPE Total use of renewable primary energy resources; NRPE Non renewable primary
energy resources used as energy carrier; NRPM Non renewable primary energy resources used as materials;
TRPE Total use of non renewable primary energy resources; SM Use of secondary materials; RSF Use of
renewable secondary fuels; NRSF Use of non renewable secondary fuels; W Use of net fresh water.
8/11
NEPD-2742-1440-EN PAROC Stone Wool Thermal Insulation (Ultra)
LCA: Results
End of Life – Waste: 1m2 PAROC Ultra (per 1,13 kg)
Parameter Unit A 1-3 A4 A5 C2 C4 D
HW [kg] 2,96E-008 3,32E-008 1,73E-011 2,41E-009 3,44E-009 -3,07E-010
NHW [kg] 0,145 0,00109 0,000778 7,91E-006 1,14 -0,000349
RW [kg] 0,000229 8,84E-007 1,27E-006 6,4E-008 2,57E-006 -5,54E-005
HW Hazardous waste disposed; NHW Nonhazardous waste disposed; RW Radioactive waste disposed.
End of Life – Output Flow: 1m2 PAROC Ultra (per 1,13 kg)
Parameter Unit A 1-3 A4 A5 C2 C4 D
CR [kg] 0 0 0 0 0 0
MR [kg] 0 0 0 0 0 0
MER [kg] 0 0 0,0602 0 0 0
EEE [MJ] 0 0 0,185 0 0 0
ETE [MJ] 0 0 0,359 0 0 0
CR Components for reuse; MR Materials for recycling; MER Materials for energy recovery; EEE Exported electric
energy; ETE Exported thermal energy.
Key environmental Unit Cradle to gate Transport
indicators A1-A3 ****
Global Warming kg C0 -eqv 1,26 0,05
2
Energy Use (=TPE+TRPE) MJ 13,64 -
Dangerous substances * - -
*The product contains no substances from the REACH Cand idate list of the Norwegian priority list.
****Average transport from production site to customer.
9/11
NEPD-2742-1440-EN PAROC Stone Wool Thermal Insulation (Ultra)
Additional Norwegian Requirements
Greenhouse gas emissions from the use of electricity in the manufacturing phase
The selection of the background data for the electricity generation is in line with EN 15804 and contribute to GWP
as given below.
G reenhouse gas emissions
Country Amount Unit
Lithuania 0,421 kg CO -eqv/kWh
2
Dangerous substances
☒ The product contains no substances given by the REACH Candidate list or the
Norwegian priority list. The product is classified as hazardous waste (Avfallsforskiften,
Annex III), see table.
☐ The product contains substances given by the REACH Candidate list or the Norwegian
priority list that are less than 0,1 % by weight.
☐ The product contains dangerous substances, more then 0,1% by weight, given by the
REACH Candidate List or the Norwegian Priority list, see table.
☐ The product contains no substances given by the REACH Candidate list or the
Norwegian priority list. The product is classified as hazardous waste (Avfallsforskiften,
Annex III), see table.
Dangerous substances
None of the following substances have been added to the product: Substances on the REACH Candidate list of
substances of very high concern or substances on the Norwegian Priority list as of 15.01.2019 or substances that
lead to the product being classified as hazardous waste. The chemical content of the product complies with regulatory
levels as given in the Norwegian Product Regulations.
Transport
Average transport distance from production site to customer is: 450 km
Carbon footprint
Carbon footprint has not been worked out for the product.
10/11
NEPD-2742-1440-EN PAROC Stone Wool Thermal Insulation (Ultra)
Bibliography
ISAOd d14it0i2o5n:2a0l1 N0 o rwegian RequiremenEtnsv ironmental labels and declarations – Type III environmental
declarations – Principles and procedures.
ISO 14040:2006 Environmental management – Life cycle assessment – Principles and
framework.
ISO 14044:2006 Environmental management – Life cycle assessment – Requirements
and guidelines.
EN 15804:2012+A1:2013 Sustainability of construction works – Environmental product
declaration – Core rules for the product category of construction
products.
ISO 21930:2007 Sustainability in building construction – Environmental declaration of
building products.
Dr. Iris Matzke, Yannick Bernard Background report for EPD of Paroc Stone Wool Insulation.
September 2020, revised March 2021.
PCR NPCR 012:2018 version 2. Part B for Thermal insulation products
Program Operator and Publish Phone +47 23 08 80 00
The Norwegian EPD Foundation
Post Box 5250 Majorstuen, 0303 Oslo e-mail: post@epd-norge.no
Norway web: www.epd-norge.no
Owner of the declaration Phone +358 46 876 8000
Paroc Group Oy
FI-00181, Helsinki e-mail: paroc.communication@owenscorning.com
Finland web: www.paroc.com
Sphera Solutions GmbH Phone: +49 (0) 711 34 18 17-0
Yannick Bernard Fax +49 (0) 711 34 18 17-25
Hauptsraße 111-113 e-mail: info@sphera.com
70771 Leinfelden-Echterdingen web: www.sphera.com
11/11
NEPD-2742-1440-EN PAROC Stone Wool Thermal Insulation (Ultra)
