Environmental product declaration
In accordance with ISO 14025 and EN15804+A2
ArcelorMittal Construction organic coated low profiles
Owner of the declaration: Program operator:
ArcelorMittal Construction Norge AS The Norwegian EPD Foundation
Product: Declaration number:
ArcelorMittal Construction organic coated low profiles
NEPD-5885-4611-EN
Declared unit:
1 kg Registration number:
This declaration is based on Product Category Rules: NEPD-5885-4611-EN
CEN Standard EN 15804:2012+A2:2019 serves as core
Issue date: 25.01.2024
PCR
The Norwegian EPD Foundation
NPCR 013:2021 Part B for Steel and aluminium Valid to: 25.01.2029
construction products
EPD Software:
LCA.no EPD generator ID: 63666
1 / 12
General information
Product Owner of the declaration:
ArcelorMittal Construction organic coated low profiles ArcelorMittal Construction Norge AS
Contact person: Stig Tore Sjaastad
Phone: +47 41 723939
e-mail: stig-tore.sjaastad@arcelormittal.com
Program operator: Manufacturer:
Post Box 5250 Majorstuen, 0303 Oslo, Norway ArcelorMittal Construction Sverige AB
The Norwegian EPD Foundation Västanvindsgatan 13
Phone: +47 23 08 80 00 SE-652 21 Karlstad, Sweden
web: post@epd-norge.no
Declaration number: Place of production:
ArcelorMittal Construction Sverige AB - Karlstad
NEPD-5885-4611-EN
Västanvindsgatan 13
SE-652 21 Karlstad, Sweden
This declaration is based on Product Category Rules: Management system:
CEN Standard EN 15804:2012+A2:2019 serves as core PCR ISO 9001, ISO 14001, ISO 45001
NPCR 013:2021 Part B for Steel and aluminium construction products
Statement of liability: Organisation no:
The owner of the declaration shall be liable for the underlying 976289862
information and evidence. EPD Norway shall not be liable with respect
to manufacturer information, life cycle assessment data and
evidences.​
Declared unit: Issue date: 25.01.2024
1 kg ArcelorMittal Construction organic coated low profiles
Declared unit with option: Valid to: 25.01.2029
A1-A3,A4,A5,C1,C2,C3,C4,D
Year of study:
2022
Functional unit: Comparability:
EPD of construction products may not be comparable if they not
comply with EN 15804 and seen in a building context.
General information on verification of EPD from EPD tools: Development and verification of EPD:
Independent verification of data, other environmental information The declaration is created using EPD tool lca.tools ver EPD2022.03,
and the declaration according to ISO 14025:2010, § 8.1.3 and § 8.1.4. developed by LCA.no. The EPD tool is integrated in the company's
Verification of each EPD is made according to EPD-Norway’s management system, and has been approved by EPD Norway.
guidelines for verification and approval requiring that tools are i)
integrated into the company's environmental management system, ii) Developer of EPD: Stig Tore Sjaastad
the procedures for use of the EPD tool are approved by EPD-Norway,
Reviewer of company-specific input data and EPD:​ Bendik Hovde
and iii) the process is reviewed annually by an independent third
party verifier. See Appendix G of EPD-Norway's General Programme
Instructions for further information on EPD tools
Verification of EPD tool: Approved:
Independent third party verification of the EPD tool, background data
and test-EPD in accordance with EPDNorway's procedures and
guidelines for verification and approval of EPD tools.
Third party verifier:
Alexander Borg, Asplan Viak AS
(no signature required)
2 / 12
Product
Product description:
This Environmental Product Declaration refers to organic coated steel profile produced by ArcelorMittal Construction Sweden. These products are
made of cold-rolled steel profiles for roof, wall, facades and floors applications.
The targeted applications are as follow:
- Roof & Decking
- Traditional wall
- Facade architectural
- Sidings
- Cassettes
- Wall liner trays
- Floors
These profiles are available in different thicknesses from 0.5 to 1.25 mm. They can be covered with different metallic coating with masses from 60
to 350 g/m². They are also constituted of an organic coating with thicknesses from 12 to 205 µm.
This EPD covers the following organic coated steel profiles produced by ArcelorMittal Construction Sweden:
- AM Galant 510, TP16, TP17, TP20 LS, TP20 OL, TP32, TP32R, TP45, Sinus 27 T, VP16, VP16v, VP17, VP20 LS, VP32, VP45, Sinus 27 V,
Ambassador, Solstad, Original, Cofraplus 45
Product specification
The steel grade used for these organic coated steel profiles varies from S280 to 350GD, Z275 or equivalent in Zinc Magnesium (ZM) with an
organic coated surface. Type of coating surface and the required nominal thickness of the steel sheet is depending on the specific application and
environmental conditions.
Materials kg %
Metal - Steel 1,00 100,00
Total 1,00
Packaging kg %
Packaging - Plastic 0,00 18,01
Packaging - Wood 0,02 81,99
Total incl. packaging 1,02
Technical data:
ArcelorMittal Construction organic coated low profiles fulfill the requirement of the harmonized standard of EN 1090 and all products are CE
certified. Performance data of the product in accordance with the declaration of performance EN 14782 with respect to its essential characteristics
according to EN 1090.
Market:
The main market areas are the Nordic countries.
Reference service life, product
High profiled sheets made of steel must withstand a term of protection of at least 15 years. The term of protection is the period until first slight
renewals in the surface are required, only if there is no need of frequent inspections and service. The term of protection depends on the location,
weather conditions and the quality of the coating. Profiled sheets made of steel exhibit an estimated service life of 40 – 45 years depending on Life
Cycle Assessment.
Reference service life, building or construction works
As a structural part of the building, steel profiles are expected and specified to reach the same service life as that of the building. The steel
reference service life can be up to 100 years.
LCA: Calculation rules
Declared unit:
1 kg ArcelorMittal Construction organic coated low profiles
Cut-off criteria:
All major raw materials and all the essential energy is included. The production processes for raw materials and energy flows with very small
amounts (less than 1%) are not included. These cut-off criteria do not​ apply for hazardous materials and substances.
Allocation:
3 / 12
The allocation is made in accordance with the provisions of EN 15804. Incoming energy and water and waste production in-house is allocated
equally among all products through mass allocation. Effects of primary production of recycled materials is allocated to the main product in which
the material was used. The recycling process and transportation of the material is allocated to this analysis.
Incoming energy and water and waste production in-house is allocated equally among all products through mass allocation.
Effects of primary production of recycled materials is allocated to the main product in which the material was used.
The recycling process and transportation of the material is allocated to this analysis.
Data quality:
Specific data for the product composition are provided by the manufacturer. The data represent the production of the declared product and were
collected for EPD development in the year of study. Background data is based on EPDs according to EN 15804 and different LCA databases. The
data quality of the raw materials in A1 is presented in the table below.
Materials Source Data quality Year
Packaging - Plastic ecoinvent 3.6 Database 2019
Packaging - Wood ecoinvent 3.6 Database 2019
Metal - Steel not yet published EPD YYYY
4 / 12
System boundaries (X=included, MND=module not declared, MNR=module not relevant)
Construction Beyond the system
Product stage Use stage End of life stage
installation stage boundaries
A1 A2 A3 A4 A5 B1 B2 B3 B4 B5 B6 B7 C1 C2 C3 C4 D
X X X X X MND MND MND MND MND MND MND X X X X X
System boundary:
Type of EPD: cradle to gate - with options. All relevant life cycle stages are covered.
Modules A1-A5, C2-C4 and module D were considered.
The product stages A1-A3 include the following:
• Transporting and Receiving the raw material to the fabrication plant
• All relevant production processes in the plant including energy inputs, emissions and the electricity consumptions
• Waste processing until end of waste state or disposal of any waste residues during the production of the low profile
• Production and recycling of packaging
• Manufacturing of the low profile
Additional technical information:
waR slairetam tropsnarT gnirutcafunaM tropsnarT ylbmessA e​sU ecnanetniaM riapeR tnemecalpeR tnemhsibrufeR lanoitarepO ygrene esu lanoitarepO esu retaw -eD noitcurtsnoc noitilomed tropsnarT etsaW gnissecorp lasopsiD -yrevoceR-esueR laitnetop-gnilcyceR
5 / 12
LCA: Scenarios and additional technical information
The following information describe the scenarios in the different modules of the EPD.
The construction installation stages A4-A5 include the following:
• For the transport to the construction site an assumption of an average truck trailer of 16-32 tonnes payload has been taken into consideration.
Transport distance of the finished product to the customer has been estimated with approximate 300km. All values are based on annual average
delivery data
• For the assembly stage average values been taken.
The use stages (B1-B7) and C1 have not been considered in the Life Cycle Assessment.
The end of life stage C2-C4 include the following:
• Stages C2-C4 include average assumptions, provision for all materials and transports, and use of related energy and water
• lt takes into account the sorting and shredding of after-use steel, as well as the non-recovered scrap due to sorting efficiency, which is landfilled
• Packaging waste is recycled by the customers through their waste management system
Module D (Beyond the system boundaries) is included.
Capacity utilisation Value
Transport from production place to user (A4) Distance (km) Fuel/Energy Consumption Unit
(incl. return) % (Liter/tonne)
Truck, 16-32 tonnes, EURO 6 (km) 36,7 % 300 0,043 l/tkm 12,90
Assembly (A5) Unit Value
Waste, packaging, plastic film (LDPE), to average
kg 0,00
treatment (kg) - A5, inkl. 85 km transp.
Waste, packaging, wood beam, softwood, raw,
dried, u=20%, average treatment (kg) - A5, inkl. 85 kg 0,02
km transp.
Capacity utilisation Value
Transport to waste processing (C2) Distance (km) Fuel/Energy Consumption Unit
(incl. return) % (Liter/tonne)
Truck, over 32 tonnes, EURO 6 (km) 53,3 % 80 0,023 l/tkm 1,84
Waste processing (C3) Unit Value
Materials to recycling (kg) kg 0,90
Disposal (C4) Unit Value
Waste, scrap steel, to landfill (kg) kg 0,10
Benefits and loads beyond the system
Unit Value
boundaries (D)
Substitution of primary steel with net scrap (kg) kg 0,85
6 / 12
LCA: Results
The LCA results are presented below for the declared unit defined on page 2 of the EPD document.
Environmental impact
Indicator Unit A1-A3 A4 A5 C1 C2 C3 C4 D
GWP-total kg CO2 -eq 2,82E+00 4,90E-02 2,72E-02 0 6,97E-03 0,00E+00 4,29E-04 -9,37E-01
GWP-fossil kg CO2 -eq 2,84E+00 4,90E-02 7,67E-04 0 6,97E-03 0,00E+00 4,28E-04 -9,36E-01
GWP-biogenic kg CO2 -eq -2,26E-02 2,03E-05 2,64E-02 0 2,98E-06 0,00E+00 3,64E-07 -5,16E-04
GWP-luluc kg CO2 -eq 6,70E-04 1,74E-05 1,42E-07 0 2,12E-06 0,00E+00 8,40E-08 -4,19E-04
ODP kg CFC11 -eq 1,06E-08 1,11E-08 9,20E-11 0 1,68E-09 0,00E+00 2,09E-10 -2,97E-08
AP mol H+ -eq 5,77E-03 1,41E-04 4,11E-06 0 2,24E-05 0,00E+00 4,18E-06 -4,65E-03
EP-FreshWater kg P -eq 8,54E-06 3,92E-07 6,20E-09 0 5,54E-08 0,00E+00 3,20E-09 -5,76E-05
EP-Marine kg N -eq 1,39E-03 2,79E-05 1,95E-06 0 4,91E-06 0,00E+00 1,57E-06 -9,63E-04
EP-Terrestial mol N -eq 1,48E-02 3,12E-04 1,85E-05 0 5,48E-05 0,00E+00 1,73E-05 -9,84E-03
POCP kg NMVOC -eq 5,00E-03 1,19E-04 4,86E-06 0 2,15E-05 0,00E+00 4,94E-06 -4,69E-03
ADP-minerals&metals1 kg Sb -eq 4,32E-05 1,35E-06 9,15E-09 0 1,24E-07 0,00E+00 3,79E-09 -1,62E-05
ADP-fossil1 MJ 2,84E+01 7,41E-01 6,71E-03 0 1,13E-01 0,00E+00 1,38E-02 -7,88E+00
WDP1 m3 2,95E+01 7,17E-01 1,28E-02 0 8,68E-02 0,00E+00 2,91E-02 4,85E+01
GWP-total = Global Warming Potential total; GWP-fossil = Global Warming Potential fossil fuels; GWP-biogenic = Global Warming Potential biogenic; GWP-luluc =
Global Warming Potential land use and land use change; ODP = Depletion potential of the stratospheric ozone layer; AP = Acidification potential, Accumulated
Exceedance; EP-freshwater = Eutrophication potential, fraction of nutrients reaching freshwater end compartment: EP-marine = Eutrophication potential, fraction of
nutrients reaching marine end compartment; EP-terrestrial = Eutrophication potential, Accumulated Exceedance; POCP = Formation potential of tropospheric ozone;
ADP-minerals&metals = Abiotic depletion potential for non-fossil resources; ADP-fossil = Abiotic depletion for fossil resources potential; WDP = Water (user)
deprivation potential, deprivation-weighted water consumption
"Reading example: 9,0 E-03 = 9,0*10-3 = 0,009"
*INA Indicator Not Assessed
1. The results of this environmental impact indicator shall be used with care as the uncertainties on these results are high or as there is limited experienced with the
indicator
Remarks to environmental impacts
7 / 12
Additional environmental impact indicators
Indicator Unit A1-A3 A4 A5 C1 C2 C3 C4 D
PM Disease incidence 4,35E-09 3,00E-09 5,30E-11 0 6,40E-10 0,00E+00 8,90E-11 -7,77E-08
IRP2 kgBq U235 -eq 1,49E-02 3,24E-03 2,54E-05 0 4,95E-04 0,00E+00 6,00E-05 3,36E-03
ETP-fw1 CTUe 1,62E+00 5,49E-01 7,41E-03 0 8,28E-02 0,00E+00 6,83E-03 -5,22E+01
HTP-c1 CTUh 1,10E-11 0,00E+00 1,00E-12 0 0,00E+00 0,00E+00 0,00E+00 -4,50E-09
HTP-nc1 CTUh 2,08E-09 6,00E-10 3,40E-11 0 8,00E-11 0,00E+00 4,00E-12 9,79E-08
SQP1 dimensionless 2,17E+00 5,18E-01 5,23E-03 0 1,30E-01 0,00E+00 5,04E-02 -5,89E-01
PM = Particulate Matter emissions; IRP = Ionizing radiation – human health; ETP-fw = Eco toxicity – freshwater; HTP-c = Human toxicity – cancer effects; HTP-nc =
Human toxicity – non cancer effects; SQP = Potential Soil Quality Index (dimensionless)
"Reading example: 9,0 E-03 = 9,0*10-3 = 0,009"
*INA Indicator Not Assessed
1. The results of this environmental impact indicator shall be used with care as the uncertainties on these results are high or as there is limited experienced with the
indicator
2. This impact category deals mainly with the eventual impact of low dose ionizing radiation on human health of the nuclear fuel cycle. It does not consider effects due
to possible nuclear accidents, occupational exposure nor due to radioactive waste disposal in underground facilities. Potential ionizing radiation from the soil, from
radon and from some construction materials is also not measured by this indicator.
8 / 12
Resource use
Indicator Unit A1-A3 A4 A5 C1 C2 C3 C4 D
PERE MJ 1,51E+00 1,06E-02 1,44E-04 0 1,42E-03 0,00E+00 2,13E-04 -6,39E-01
PERM MJ 2,42E-01 0,00E+00 -2,42E-01 0 0,00E+00 0,00E+00 0,00E+00 0,00E+00
PERT MJ 1,75E+00 1,06E-02 -2,42E-01 0 1,42E-03 0,00E+00 2,13E-04 -6,39E-01
PENRE MJ 2,84E+01 7,41E-01 6,71E-03 0 1,13E-01 0,00E+00 1,38E-02 -7,87E+00
PENRM MJ 1,61E-01 0,00E+00 -1,61E-01 0 0,00E+00 0,00E+00 0,00E+00 0,00E+00
PENRT MJ 2,85E+01 7,41E-01 -1,55E-01 0 1,13E-01 0,00E+00 1,38E-02 -7,87E+00
SM kg 5,15E-02 0,00E+00 0,00E+00 0 0,00E+00 0,00E+00 0,00E+00 0,00E+00
RSF MJ 1,28E-02 3,79E-04 4,10E-06 0 4,98E-05 0,00E+00 4,39E-06 3,38E-02
NRSF MJ 5,61E-03 1,36E-03 3,95E-05 0 1,67E-04 0,00E+00 1,26E-05 9,84E-01
FW m3 7,03E-03 7,92E-05 4,64E-06 0 1,29E-05 0,00E+00 1,65E-05 -1,97E-03
PERE = Use of renewable primary energy excluding renewable primary energy resources used as raw materials; PERM = Use of renewable primary energy resources used
as raw materials; PERT = Total use of renewable primary energy resources; PENRE = Use of non renewable primary energy excluding non-renewable primary energy
resources used as raw materials; PENRM = Use of non renewable primary energy resources used as raw materials; PENRT = Total use of non renewable primary energy
resources; SM = Use of secondary materials; RSF = Use of renewable secondary fuels; NRSF = Use of non-renewable secondary fuels; FW = Net use of fresh water
"Reading example: 9,0 E-03 = 9,0*10-3 = 0,009"
*INA Indicator Not Assessed
9 / 12
End of life - Waste
Indicator Unit A1-A3 A4 A5 C1 C2 C3 C4 D
HWD kg 2,48E-04 3,82E-05 0,00E+00 0 6,19E-06 0,00E+00 0,00E+00 -4,87E-03
NHWD kg 7,84E-02 3,60E-02 2,11E-02 0 9,84E-03 0,00E+00 1,00E-01 -3,83E-01
RWD kg 7,89E-04 5,05E-06 0,00E+00 0 7,73E-07 0,00E+00 0,00E+00 2,58E-06
HWD = Hazardous waste disposed; NHWD = Non-hazardous waste disposed; RWD = Radioactive waste disposed
"Reading example: 9,0 E-03 = 9,0*10-3 = 0,009"
*INA Indicator Not Assessed
End of life - Output flow
Indicator Unit A1-A3 A4 A5 C1 C2 C3 C4 D
CRU kg 0,00E+00 0,00E+00 0,00E+00 0 0,00E+00 0,00E+00 0,00E+00 0,00E+00
MFR kg 4,30E-02 0,00E+00 1,94E-03 0 0,00E+00 9,00E-01 0,00E+00 0,00E+00
MER kg 0,00E+00 0,00E+00 1,73E-02 0 0,00E+00 0,00E+00 0,00E+00 0,00E+00
EEE MJ 0,00E+00 0,00E+00 1,20E-02 0 0,00E+00 0,00E+00 0,00E+00 0,00E+00
EET MJ 0,00E+00 0,00E+00 1,82E-01 0 0,00E+00 0,00E+00 0,00E+00 0,00E+00
CRU = Components for re-use; MFR = Materials for recycling; MER = Materials for energy recovery; EEE = Exported energy electrical; EET = Exported energy thermal
"Reading example: 9,0 E-03 = 9,0*10-3 = 0,009"
*INA Indicator Not Assessed
Biogenic Carbon Content
Indicator Unit At the factory gate
Biogenic carbon content in product kg C 0,00E+00
Biogenic carbon content in accompanying packaging kg C 7,21E-03
Note: 1 kg biogenic carbon is equivalent to 44/12 kg CO2
10 / 12
Additional requirements
Greenhouse gas emissions from the use of electricity in the manufacturing phase
National production mix from import, low voltage (production of transmission lines, in addition to direct emissions and losses in grid) of applied
electricity for the manufacturing process (A3).
Electricity mix Data source Amount Unit
Electricity, Sweden (kWh) ecoinvent 3.6 54,94 g CO2-eq/kWh
Dangerous substances
The product contains no substances given by the REACH Candidate list.
Indoor environment
Additional Environmental Information
Additional environmental impact indicators required in NPCR Part A for construction products
Indicator Unit A1-A3 A4 A5 C1 C2 C3 C4 D
GWPIOBC kg CO2 -eq 2,84E+00 4,90E-02 2,69E-02 0 6,97E-03 0,00E+00 0,00E+00 -1,40E+00
GWP-IOBC: Global warming potential calculated according to the principle of instantaneous oxidation. In order to increase the transparency of biogenic carbon​
contribution to climate impact, the indicator GWP-IOBC is required as it declares climate impacts calculated according to the principle of instantaneous oxidation.​
GWP-IOBC is also referred to as GWP-GHG in context to Swedish public procurement legislation.
11 / 12
Bibliography
ISO 14025:2010 Environmental labels and declarations - Type III environmental declarations - Principles and procedures.
ISO 14044:2006 Environmental management - Life cycle assessment - Requirements and guidelines.
EN 15804:2012+A2:2019 Environmental product declaration - Core rules for the product category of construction products.
ISO 21930:2017 Sustainability in buildings and civil engineering works - Core rules for environmental product declarations of construction
products.
ecoinvent v3, Allocation, cut-off by classification, Swiss Centre of Life Cycle Inventories.
Iversen et al., (2021) eEPD v2021.09 Background information for EPD generator tool system verification, LCA.no Report number: 07.21
Graafland and Iversen, (2022) EPD generator for EPD generator for NPCR 013 Part B for Steel and Aluminum, Background information for EPD
generator application and LCA data, LCA.no report number: 08.22
NPCR Part A: Construction products and services. Ver. 2.0. April 2021, EPD-Norge.
NPCR 013 Part B for Steel and Aluminium Construction Products , Ver. 4.0, 06.10.2021, EPD Norway.
Program operator and publisher Phone: +47 23 08 80 00
The Norwegian EPD Foundation e-mail: post@epd-norge.no
Post Box 5250 Majorstuen, 0303 Oslo, Norway web: www.epd-norge.no
Owner of the declaration: Phone: +47 41 723939
stig-
ArcelorMittal Construction Norge AS e-mail:
tore.sjaastad@arcelormittal.com
Sørumgata 11A, 2000 Lillestrøm web:
Author of the Life Cycle Assessment Phone: +47 916 50 916
LCA.no AS e-mail: post@lca.no
Dokka 6B, 1671 web: www.lca.no
Developer of EPD generator Phone: +47 916 50 916
LCA.no AS e-mail: post@lca.no
Dokka 6B,1671 Kråkerøy web: www.lca.no
ECO Platform web: www.eco-platform.org
ECO Portal web: ECO Portal
12 / 12
