1114 NEPD
Ver. 2 2015(17)
ENVIRONMENTAL PRODUCT DECLARATION
in accordance with ISO 14025, ISO 21930 and EN 15804
Owner of the declaration: Flügger Norway AS
Program operator: The Norwegian EPD Foundation
Publisher: The Norwegian EPD Foundation
Declaration number: NEPD-2666-1373-EN
Registration number: NEPD-2666-1373-EN
ECO Platform reference number: -
Issue date: 08.02.2021
Valid to: 08.02.2026
Fiona Adhesive 270 WallpaperTM
Flügger Norway AS
www.epd-norge.no
Add Product Picture
NEPD-2666-1373-EN Fiona Adhesive 270 WallpaperTM
General information
Product: Owner of the declaration:
Fiona Adhesive 270 WallpaperTM Flügger Norway AS
contact person: Stine Rosendal Tangaa
phone: +45 40 64 75 98
e-mail: regulatoryaffairs@flugger.com
Program operator: Manufacturer:
The Norwegian EPD Foundation Flügger Denmark A/S
Pb. 5250 Majorstuen, 0303 Oslo
Tlf: +47 23 08 82 92
e-post: post@epd-norge.no
Declaration number: Place of production:
NEPD-2666-1373-EN Vejlevej 150,
6000 Kolding, Denmark
ECO Platform reference number: Management system:
ISO 14001:2015 (DK011198)
ISO 9001:2015 (DK0012451)
This declaration is based on PCR: Org. no.:
NS-EN 15804:2012+A1:2013 serves as core PCR. 45240118
Product descriptions based on "IBU PCR Part B for coatings
with organic binders". This also applies to products with
inorganic binders.
Issue date:
Statement of liability: 08.02.2021
The owner of the declaration shall be liable for the underlying
informationandevidence.EPDNorwayshallnotbeliablewith
respect to manufacturer information, life cycle assessment
data and evidences. Valid to:
08.02.2026
Declared unit: Year of study:
2019
1 kg Fiona Adhesive 270 Wallpaper delivered to market
Declared unit with option: Comparability:
EPD of construction products may not be comparable if they
do not comply with NS-EN 15804 and seen in a building
context.
Functional unit: Author of the Life Cycle Assessment:
Mafalda Silva
NORSUS
Verification:
Independent verification of data, other environmental
information and the declaration according to ISO14025:2010, §
8.1.3 and § 8.1.4
internal external
Approved
Third party verifier:
Erik Svanes, Senior Researcher
(Independent verifier approved by EPD Norway)
NEPD-2666-1373-EN Fiona Adhesive 270 WallpaperTM 2/9
Product
Product description: Technical data:
Fiona Adhesive 270 Wallpaper is a ready-mixed, transparent, Density: 1,03 kg/l
reinforced adhesive. For indoor use in a dry room for hanging Solids by volume: 12,0%
sawdust wallpaper, paper wallpaper and non-woven wallpaper.
Nominal spreading rate: 4-6 m2/l
Fiona Adhesive 270 Wallpaper is ecolabelled with the Nordic Dilution: Water (should not normally be diluted)
Ecolabel.
The product packaging is based on an average sized plastic
For information on Green Building Standard credits and Ecolabels, packaging and is reported in the A1-phase.
see "Additional Information" on page 4.
For information on technical data, application and use of the
product, see the Technical Data Sheet and FDV (Forvaltning,
Drift og Vedlikehold) for the declared product on
www.flugger.no
Product specification:
The product is only made in one colour and has no variation in
For safety, health and environmental conditions, see the
composition.
Safety Data Sheet for the declared product on
www.flugger.no.
The material composition of the declared product:
Materials % Market:
Water 85-90 Scandinavia and Europe
Binder 1-3
Extender 5-10 Reference service life, product
Solvent 0 The reference service life of the product is highly dependent
Additive 1-3 on the conditions of use.
Biocide <0.5
Estimated service life, object
Packaging kg The coated object is not declared.
Wooden packaging - pallet 4,90E-02
Plastic packaging - pallet 1,71E-03
Plastic packaging 3,42E-02
LCA: Calculation rules
Declared unit: System boundary:
1 kg Fiona Adhesive 270 Wallpaper delivered to market The flow chart below illustrates the system boundaries for the
analysisaccordingtothemoduleprincipleinNS-EN15804.The
analysis is carried out from cradle-to-gate (A1-A3), including
module A4 transport to market.
A1 A2 A3 A4 A5 B1-B7 C1-C4 D
Raw materials Transport Production Transport to Application and Usephase Endof life Benefits of
market installation recovery
Preassemblyof
raw materials
Rawmaterial Transport of
extraction and raw materials
production Dispersionof
pigments
Transportof Module not Module not Module not Module not
product to declared declared declared declared
market
Mixing
Packaging Transport of
production packaging
QCcheck and
adjustment
Fillingand
labelling
Systemboundaries«Cradle-to-gate»
System boundary for this EPD
NEPD-2666-1373-EN Fiona Adhesive 270 WallpaperTM 3/9
System boundary for this EPD
Data quality:
The CEPE database is used as basis for the rawmaterial composition. Specific datafor theproduct composition and rawmaterial
amounts has been provided bythe manufacturer and represents the production of the declared product. Production site data was
collected in 2020, with 2019 as reference year. Remaining data is based on Ecoinvent v3.6, but adjusted to improve
representativeness. All energy consumption in the database is assumed not to be used as raw material.
Cut-off criteria: Allocation:
All major raw materials and essential energy is included. The Theallocationismadeinaccordancewiththeprovisionsof
production process for raw materials and energy flows with very NS-EN 15804. Incoming energy, water and waste
small amounts (<1%), such as consumables in production and productionin-houseisprimarilyallocatedequallyamongall
administrationandemployeetravel,arenotincluded.Thesecut-off products through volume allocation. The recycling process
criteria do not apply for hazardous materials and substances. and transportation of the material is allocated to this
analysis.
Additional information:
The declared product contributes to Green Building Standard credits by meeting the following specific requirements:
-Nordic Swan Ecolabel (3097 0008)
-Properties criteria in BASTA (2020:A2)
-Accepted according to Byggvarubedömningens Assessment Criteria 5.0 (2019)
-Class B according to SundaHus Material Data Assessment Criteria 6.1.5 (2019)
BREEAM®NOR (2016)
HEA 02: The VOC-Directive does not cover adhesives (EU Directive 2004/42/CE).
Mat01:TheproductcontainsnosubstancesontheNorwegianTechnicalCheckList(A20),whichexceedsthelimitvalueforhealthand
environment.
Additional certificates and approvals may be available on request.
NEPD-2666-1373-EN Fiona Adhesive 270 WallpaperTM 4/9
LCA: Scenarios and additional technical information
The following information describe the scenarios in the different modules of the EPD.
The only declared module after the factory gate is A4 transport to market.
Transport from production place to user (A4)
Capacity utilisation Fuel/Energy
Type Type of vehicle Distance km Unit
incl. return [%] consumption
Truck 53 >32t, EURO 6 537 1,92E-02 kg/tkm
Truck 53 >32t, EURO 6 338 1,92E-02 kg/tkm
Truck 26 16-32t, EURO 6 30 4,80E-02 kg/tkm
Construction/Installation (A5) Use (B1)
Unit Value Unit Value
Auxiliary kg Relevant emissions during use kg
Water consumption m3
Electricity consumption kWh
Other energy carriers MJ
Material loss kg
Dust in the air kg
VOC emissions kg
Maintenance (B2)/Repair (B3) Replacement (B4)/Refurbishment (B5)
Unit Value Unit Value
Maintenance cycle* Replacement cycle* pcs
Auxiliary kg Electricity consumption kWh
Other resources kg Replacement of worn parts 0
Water consumption m3 * Value or refence shelf-life
Electricity consumption kWh
Other energy carriers MJ
Material loss kg
VOC emissions kg
Operational energy (B6) and water consumption (B7) End of life (C1, C3, C4)
Unit Value Unit Value
Water consumption m3 Hazardous waste disposed kg
Electricity consumption kWh Collected as mixed construction waste kg
Other energy carriers MJ Reuse kg
Power output of equipment kW Recycling kg
Energy recovery kg
For landfill kg
Transport to waste processing (C2)
Capacity utilisation (incl. Fuel/Energy
Type Type of vehicle Distance km Unit Value (l/t)
return) % consumption
Truck
Railway
Boat
Other
NEPD-2666-1373-EN Fiona Adhesive 270 WallpaperTM 5/9
LCA: Results
System boundaries (X=included, MND=module not declared, MNR=module not relevant)
C1 C3 C4 D
MND MND
Environmental impact
A2 A3 A4
8,42E-03 1,53E-01 8,03E-02
5,78E-08 1,56E-09 1,02E-08
1,14E-06 6,92E-05
1,40E-03
1,35E-04
tnemecalpeR
A5 B7
MND MND
A1
3,54E-01
1,58E-08
1,34E-04 1,01E-05
tropsnarT
MND
Parameter
GWP kg CO -eq. 2
esu
retaw
lanoitarepO
A2 A3 A4 B2 B3 B4 B5 C2
X X X MND MND MND MND MND
Unit
kg CFC11-eq.
tropsnarT
/noitcurtsnoC egats
noitallatsni esU
Construction/
installation stage
slairetam
waR
Product stage
-gnilcycer/yrevocer/esueR
laitnetop
End of life stage
gnirutcafunaM tnemhsibrufeR
noitilomed
/noitcurtsnoceD
gnissecorp
etsaW
lasopsid
etsaW
Beyond the
system
boundaries
A1 B1 B6
X MND
ODP
POCP kg CH -eq. 2 4
AP kg SO 2 -eq. 1,85E-03 2,73E-05 2,10E-04
EP kg PO 43--eq. 3,92E-04 4,42E-06 2,82E-05
ADPM kg Sb -eq. 3,38E-06 2,12E-07 3,50E-05 1,49E-06
ADPE MJ 8,86E+00 1,27E-01 1,53E+00 1,29E+00
GWP Global warming potential; ODP Depletion potential of the stratospheric ozone layer; POCP Formation potential of tropospheric
photochemical oxidants; AP Acidification potential of land and water; EP Eutrophication potential; ADPM Abiotic depletion potential for non fossil
resources; ADPE Abiotic depletion potential for fossil resources
tropsnarT
MND
ecnanetniaM
riapeR
esu
ygrene
lanoitarepO
User stage
MND
NEPD-2666-1373-EN Fiona Adhesive 270 WallpaperTM 6/9
Resource use
Parameter Unit A1 A2 A3 A4
RPEE MJ 2,77E+00 1,85E-03 7,77E-01 1,67E-02
RPEM MJ 0,00E+00 0,00E+00 3,25E-02 0,00E+00
TPE MJ 2,77E+00 1,85E-03 8,09E-01 1,67E-02
NRPE MJ 3,02E+00 1,30E-01 1,94E+00 1,31E+00
NRPM MJ 6,61E+00 0,00E+00 0,00E+00 0,00E+00
TRPE MJ 9,63E+00 1,30E-01 1,94E+00 1,31E+00
SM kg 0,00E+00 0,00E+00 0,00E+00 0,00E+00
RSF MJ 0,00E+00 0,00E+00 0,00E+00 0,00E+00
NRSF MJ 0,00E+00 0,00E+00 0,00E+00 0,00E+00
W m3 7,76E-03 2,46E-05 1,90E-03 2,70E-04
RPEERenewableprimaryenergyresourcesusedasenergycarrier;RPEMRenewableprimaryenergyresourcesusedasrawmaterials;TPE
Total use of renewable primary energy resources; NRPE Non renewable primary energy resources used as energy carrier; NRPM Non
renewable primary energy resources used as materials; TRPE Total use of non renewable primary energyresources; SM Use of secondary
materials; RSF Use of renewable secondary fuels; NRSF Use of non renewable secondary fuels; W Use of net fresh water
End of life - Waste
Parameter Unit A1 A2 A3 A4
HW kg 8,37E-06 3,31E-07 4,67E-04 3,20E-06
NHW kg 1,12E-01 9,03E-03 2,32E-01 1,18E-01
RW kg 2,62E-05 8,83E-07 7,69E-06 8,96E-06
HW Hazardous waste disposed; NHW Non hazardous waste disposed; RW Radioactive waste disposed
End of life - Output flow
Parameter Unit A1 A2 A3 A4
CR kg 0,00E+00 0,00E+00 0,00E+00 0,00E+00
MR kg 0,00E+00 0,00E+00 9,18E-03 0,00E+00
MER kg 0,00E+00 0,00E+00 4,38E-05 0,00E+00
EEE MJ 0,00E+00 0,00E+00 3,11E-03 0,00E+00
ETE MJ 0,00E+00 0,00E+00 3,33E-02 0,00E+00
CR Components for reuse; MR Materials for recycling; MER Materials for energy recovery; EEE Exported electric energy; ETE Exported thermal
energy
Reading example: 9,0 E-03 = 9,0*10-3 = 0,009
NEPD-2666-1373-EN Fiona Adhesive 270 WallpaperTM 7/9
Additional requirements
Greenhouse gas emissions from the use of electricity in the manufacturing phase
Nationalproductionmixfromimport,lowvoltage(productionoftransmissionlines,inadditiontodirectemissionsandlossesingrid)
of applied electricity for the manufacturing process (A3). Background data is presented inthe tablebelow. Characterisationfactors
from NS-EN 15804:2012+A1:2013 is used.
Electricity mix Data source Value Unit
Electricity, Denmark (kWh) ecoinvent 3.6 329 g CO -eq./kWh
2
Dangerous substances
The product contains no substances given by the REACH Candidate list or the Norwegian priority list
The product contains substances given by the REACH Candidate list <0,1 weight%
The product contains substances given by the REACH Candidate list or the Norwegian priority list, see table above
The product contains no substances given by the REACH Candidate list or the Norwegian priority list. The product is
characterised as hazardous waste (acc. to the Waste Directive, Appendix III), se table above.
Indoor environment
The declared product is emission tested according to the ISO-16000 series (2006).
NEPD-2666-1373-EN Fiona Adhesive 270 WallpaperTM 8/9
Bibliography
BASTA (2020) Properties criteria - BASTA - in accordance with Regulation (EC) No 1272/2008 (CLP), ed. A2
BREEAM®NOR (2016) BREEAM-NOR for new contractions 2016, SD5075NOR, version 1.1. The Norwegian Green Building
Council
Byggvarubedömningen (2019) Assessment criteria for chemical content and lifecycle aspects, version 5.0
CEPE (2016) Raw materials LCI database for the European coatings and printing ink industries, v3.0
Ecoinvent (2019) Ecoinvent version 3.6, Swiss Centre of Life Cycle Inventories, Dübendorf, Switzerland
EU Directive 2004/42/CE The limitation of emissions of volatile organic compounds due to the use of organic solvents in
certain paints and varnishes and vehicle refinishing products
IBU PCR Part B Requirements on the EPD for Coatings with organic binders. v1.7, January 2019
ISO 14025:2010 Environmental labels and declarations - Type III environmental declarations - Principles and
procedures
ISO 16000-series Indoor air standards for VOCs sampling and determination, i.e. 9 (2006)
ISO 21930:2017 Sustainability in buildings and civil engineering works - Core rules for environmental product
declarations of construction products and services
NS-EN 15804:2012+A1:2013 Environmental product declaration - Core rules for the product category of construction products
REACH Candidate List (2018) Candidate List of substances of very high concern for Authorisation IAW Article 59(10) of the REACH
Regulation
SundaHus (2019) Material Data Assessment Criteria, version 6.1.5
Nordic Ecolabel 3097 0008 - Fiona Adhesive 270 Wallpaper.
Technical Check List (A20) and Miljøgiftlisten, The Norwegian Environment Agency
Norwegian Priority List (2018)
Program operator and publisher phone: +47 977 22 020
The Norwegian EPD Foundation
Post Box 5250 Majorstuen, 0303 Oslo e-mail: post@epd-norge.no
Norway web www.epd-norge.no
Owner of the declaration phone: +47 23 30 21 90
Flügger Norway AS
Waldemar Thranes gate 84B e-mail: regulatoryaffairs@flugger.com
0175 Oslo, Norway web www.flugger.com
Author of the Life Cycle Assessment phone: +47 69 35 11 00
Mafalda Silva, Lars Tellnes & Gaylord Booto fax: +47 69 34 24 94
NORSUS AS e-mail: post@norsus.no
Stadion 4, 1671 Kråkerøy, Norge web www.norsus.no
NEPD-2666-1373-EN Fiona Adhesive 270 WallpaperTM 9/9
