Environmental product declaration
in accordance with ISO 14025 and EN 15804+A2
Hvalpsund Extreme 500NG
Owner of the declaration: Program operator:
Mørenot Aquaculture AS The Norwegian EPD Foundation
Product: Declaration number:
Hvalpsund Extreme 500NG NEPD-7160-6556-EN
Declared unit: Registration number:
1 pcs NEPD-7160-6556-EN
This declaration is based on Product Category Rules: Issue date:
CEN Standard EN 15804:2012+A2:2019 serves as core 26.07.2024
PCR
The Norwegian EPD Foundation Valid to:
NPCR 031:2023 Part B for sea-based aquaculture
26.07.2029
infrastructure and components
EPD software:
LCAno EPD generator ID: 447431
1 / 11
General information
Product Owner of the declaration:
Hvalpsund Extreme 500NG Mørenot Aquaculture AS
Contact person: Liv Lund
Phone: +4792032311
e-mail: liv.lund@morenot.com
Program operator: Manufacturer:
The Norwegian EPD Foundation Mørenot Aquaculture AS
Post Box 5250 Majorstuen, 0303 Oslo, Norway
Phone: +47 977 22 020
web: www.epd-norge.no
Declaration number: Place of production:
Mørenot Aquaculture AS
NEPD-7160-6556-EN
Langelandsvegen 35
6010 Ålesund, Norway
This declaration is based on Product Category Rules: Management system:
CEN Standard EN 15804:2012+A2:2019 serves as core PCR ISO9001 and ISO14001
NPCR 031:2023 Part B for sea-based aquaculture infrastructure and
components
Statement of liability: Organisation no:
The owner of the declaration shall be liable for the underlying 997749588
information and evidence. EPD Norway shall not be liable with respect
to manufacturer information, life cycle assessment data and
evidences.​
Declared unit: Issue date:
1 pcs Hvalpsund Extreme 500NG 26.07.2024
Declared unit with option: Valid to:
A1,A2,A3,A4,C1,C2,C3,C4,D 26.07.2029
Year of study:
2023
Functional unit: Comparability:
Floating structure that keeps the fish cage in the surface of the sea EPD of construction products may not be comparable if they not
and the net in place. comply with EN 15804 and seen in a building context.
General information on verification of EPD from EPD tools: Development and verification of EPD:
Independent verification of data, other environmental information The declaration is created using EPD tool lca.tools ver EPD2022.03,
and the declaration according to ISO 14025:2010, § 8.1.3 and § 8.1.4. developed by LCA.no. The EPD tool is integrated in the company's
Verification of each EPD is made according to EPD-Norway’s management system, and has been approved by EPD Norway.
guidelines for verification and approval requiring that tools are i)
integrated into the company's environmental management system, ii) Developer of EPD: Ingrid Johanne Høydal
the procedures for use of the EPD tool are approved by EPD-Norway,
Reviewer of company-specific input data and EPD:​ Liv Lund
and iii) the process is reviewed annually by an independent third
party verifier. See Appendix G of EPD-Norway's General Programme
Instructions for further information on EPD tools
Verification of EPD tool: Approved:
Independent third party verification of the EPD tool, background data
and test-EPD in accordance with EPDNorway's procedures and
guidelines for verification and approval of EPD tools. Approval
number: NEPDT65.
Håkon Hauan, CEO EPD-Norge
Third party verifier:
Elisabet Amat, GREENIZE projects
(no signature required)
2 / 11
Product
Product description:
Highly customisable and corrosion-free floating pens in 100% PE. Our buoyancy pens are designed and engineered to withstand extreme forces of
nature. The Hvalpsund ring has a floating pen with extra wide walkways and a non-slip surface without trip edges that helps to make the cage
edge a better and safer workplace. Hvalpsundring extreme are built in sizes from 120 to +200 mtr and the pipes comes with a diameter of
500mm.
Product specification
100% PE.
Double pipes all the way around.
Brackets made from 100% HDPE.
Materials kg %
Plastic - Polypropylene with filler 6082,68 23,35
Plastic pipe - HDPE 19972,61 76,65
Total 26055,29 100,00
Packaging kg %
Packaging - Wood 50,00 100,00
Total incl. packaging 26105,29 100,00
Technical data:
The Pen is certified according to NS-9415:2021 and NYTEK23 and are metal free.
The Hvalpsund-ring is made of 100% PE plastic and is free of steel components.
Inner floating pipe: HDPE100 Ø500 161 m SDR13,6
Outer floating pipe: HDPE100 Ø500 169 m SDR13,6
Hand rail: HDPE100 Ø140 161 m SDR11
Circumference analysed product: 160 m
Weight: 26 055, 289 kg
Market:
Norway
Reference service life, product
20 years
Reference service life, building or construction works
LCA: Calculation rules
Declared unit:
1 pcs Hvalpsund Extreme 500NG
Cut-off criteria:
All major raw materials and all the essential energy is included. The production processes for raw materials and energy flows with very small
amounts (less than 1%) are not included. These cut-off criteria do not​ apply for hazardous materials and substances.
Allocation:
The allocation is made in accordance with the provisions of EN 15804. Incoming energy and water and waste production in-house is allocated
equally among all products through mass allocation. Effects of primary production of recycled materials is allocated to the main product in which
the material was used. The recycling process and transportation of the material is allocated to this analysis.
Data quality:
Specific data for the product composition are provided by the manufacturer. The data represent the production of the declared product and were
collected for EPD development in the year of study. Background data is based on EPDs according to EN 15804 and different LCA databases. The
data quality of the raw materials in A1 is presented in the table below.
Materials Source Data quality Year
Packaging - Wood ecoinvent 3.6 Database 2019
Plastic - Polypropylene with filler ecoinvent 3.6 Database 2019
Plastic pipe - HDPE NEPD-6903-6293-EN EPD 2023
3 / 11
System boundaries (X=included, MND=module not declared, MNR=module not relevant)
Construction Beyond the system
Product stage Use stage End of life stage
installation stage boundaries
A1 A2 A3 A4 A5 B1 B2 B3 B4 B5 B6 B7 C1 C2 C3 C4 D
X X X X MND MND MND MND MND MND MND MND X X X X X
System boundary:
Additional technical information:
https://www.morenot.com/aquaculture/pens/
waR slairetam tropsnarT gnirutcafunaM tropsnarT ylbmessA e​sU ecnanetniaM riapeR tnemecalpeR tnemhsibrufeR lanoitarepO ygrene esu lanoitarepO esu retaw -eD noitcurtsnoc noitilomed tropsnarT etsaW gnissecorp lasopsiD -yrevoceR-esueR laitnetop-gnilcyceR
4 / 11
LCA: Scenarios and additional technical information
The following information describe the scenarios in the different modules of the EPD.
Module A4 - follow the default travel distance for work boats from the manufacturing site to the production location at sea is 200 Nm (370.4 km)
sea freight as stated in NPCR 031 part B if not specified to a specific customer/order.
Module C1 - Freight from the aquaculture facility to disassembly require a service vessel aquaculture operations. For the travel distance a default
sea freight of 1 Nm (1.852 km) is included to account for transport between the production location at sea and the nearest dock and is estimated
to two hours.
Module C2 - Use default distance data of 300 km for Norwegian conditions as stated in NPCR 031 part B.
Module C3-C4 - Waste treatment and the processing of waste are based upon the assumption that all material is collected at the end-of-life
phase as stated in NPCR 031 part B for aquaculture infrastructure and components. Phase C3, waste treatments include material recycling,
incineration with and without energy recovery, and fly ash extraction. In phase C4, disposal methods involve landfilling of different waste fractions
and ashes.
Capacity utilisation Value
Transport from production place to user (A4) Distance (km) Fuel/Energy Consumption Unit
(incl. return) % (Liter/tonne)
Ship, aquaculture transport, service vessel, 24
20,0 % 370 1,080 l/tkm 400,03
meters, with tugging (kgkm) - Global
De-construction demolition (C1) Unit Value
Aquaculture operation, service vessel, 24 meter,
h/DU 2,00
product de-construction (per hour) - Global
Capacity utilisation Value
Transport to waste processing (C2) Distance (km) Fuel/Energy Consumption Unit
(incl. return) % (Liter/tonne)
Truck, 16-32 tonnes, EURO 6 (km) - Europe 36,7 % 300 0,043 l/tkm 12,90
Waste processing (C3) Unit Value
Plastic compound, PP and filler, to recycling (kg) kg 2128,94
Polyethylene to recycling (kg) kg 6990,41
Waste treatment of plastic mixture, incineration
kg 3953,74
with energy recovery and fly ash extraction (kg)
Waste treatment of polyethylene (PE),
incineration with energy recovery and fly ash kg 12982,20
extraction (kg)
Waste treatment per kg of non-impregnated
aquaculture components, washing process (kg) - kg 26055,29
Norway
Disposal (C4) Unit Value
Landfilling of ashes from incineration of Plastic
kg 138,25
mixture, process per kg ashes and residues (kg)
Landfilling of ashes from incineration of
Polyethylene (PE), process per kg ashes and kg 457,51
residues (kg)
Benefits and loads beyond the system
Unit Value
boundaries (D)
Substitution of acrylonitrile butadiene styrene,
kg 638,68
ABS, granulate (kg)
Substitution of electricity, in Norway (MJ) MJ 31249,21
Substitution of Polyethylene, HDPE granulate (kg) kg 2906,82
Substitution of Polypropylene, PP granulate (kg) kg 1490,26
Substitution of thermal energy, district heating, in
MJ 472770,30
Norway (MJ)
5 / 11
LCA: Results
The LCA results are presented below for the declared unit defined on page 2 of the EPD document.
Environmental impact
Indicator Unit A1 A2 A3 A4 C1 C2 C3 C4 D
GWP-total kg CO2 -eq 6,48E+04 9,45E+01 5,32E+02 3,34E+04 6,86E+02 1,28E+03 5,07E+04 2,59E+01 -1,48E+04
GWP-fossil kg CO2 -eq 6,51E+04 9,45E+01 5,31E+02 3,34E+04 6,85E+02 1,28E+03 5,07E+04 2,59E+01 -1,46E+04
GWP-biogenic kg CO2 -eq -3,43E+02 2,60E-02 1,65E-01 6,27E+00 1,69E-01 5,28E-01 7,74E+00 1,36E-02 -6,30E+01
GWP-luluc kg CO2 -eq 3,75E+01 6,53E-02 4,21E-02 1,21E+01 4,15E-01 4,54E-01 1,46E+00 3,89E-03 -9,70E+01
ODP kg CFC11 -eq 2,47E-03 2,01E-05 1,15E-04 7,29E-03 1,47E-04 2,89E-04 3,43E-04 2,67E-06 -2,00E+02
AP mol H+ -eq 2,43E+02 3,07E+00 5,55E+00 1,15E+03 2,33E+01 3,67E+00 2,31E+01 8,91E-02 -6,40E+01
EP-FreshWater kg P -eq 1,42E+00 3,91E-04 1,94E-03 8,80E-02 2,48E-03 1,02E-02 6,28E-02 3,51E-04 -4,30E-01
EP-Marine kg N -eq 4,17E+01 7,54E-01 2,45E+00 2,78E+02 5,61E+00 7,26E-01 7,18E+00 2,77E-02 -1,44E+01
EP-Terrestial mol N -eq 4,62E+02 8,40E+00 2,69E+01 3,05E+03 6,15E+01 8,12E+00 8,13E+01 3,15E-01 -1,55E+02
POCP kg NMVOC -eq 2,08E+02 2,18E+00 7,39E+00 7,98E+02 1,62E+01 3,11E+00 2,21E+01 8,69E-02 -5,87E+01
ADP-minerals&metals1 kg Sb-eq 5,45E-01 7,02E-04 8,34E-04 1,38E-01 4,60E-03 3,53E-02 1,24E-01 1,39E-04 -1,08E-01
ADP-fossil1 MJ 2,04E+06 1,21E+03 7,31E+03 4,55E+05 9,31E+03 1,93E+04 4,33E+04 2,28E+02 -4,10E+05
WDP1 m3 5,73E+06 2,41E+02 1,57E+03 7,67E+04 1,74E+03 1,87E+04 1,99E+05 2,46E+03 -7,97E+05
GWP-total = Global Warming Potential total; GWP-fossil = Global Warming Potential fossil fuels; GWP-biogenic = Global Warming Potential biogenic; GWP-luluc =
Global Warming Potential land use and land use change; ODP = Depletion potential of the stratospheric ozone layer; AP = Acidification potential, Accumulated
Exceedance; EP-freshwater = Eutrophication potential, fraction of nutrients reaching freshwater end compartment: EP-marine = Eutrophication potential, fraction of
nutrients reaching marine end compartment; EP-terrestrial = Eutrophication potential, Accumulated Exceedance; POCP = Formation potential of tropospheric ozone;
ADP-minerals&metals = Abiotic depletion potential for non-fossil resources; ADP-fossil = Abiotic depletion for fossil resources potential; WDP = Water (user)
deprivation potential, deprivation-weighted water consumption
"Reading example: 9,0 E-03 = 9,0*10-3 = 0,009"
*INA Indicator Not Assessed
1. The results of this environmental impact indicator shall be used with care as the uncertainties on these results are high or as there is limited experienced with the
indicator
Remarks to environmental impacts
6 / 11
Additional environmental impact indicators
Indicator Unit A1 A2 A3 A4 C1 C2 C3 C4 D
PM Disease incidence 2,07E-03 0,00E+00 1,47E-04 7,97E-03 1,62E-04 7,82E-05 2,63E-04 1,09E-06 -1,75E-03
IRP2 kgBq U235 -eq 2,68E+03 5,18E+00 3,13E+01 1,98E+03 4,02E+01 8,44E+01 9,61E+01 1,09E+00 -4,44E+02
ETP-fw1 CTUe 4,55E+05 7,02E+02 4,00E+03 2,39E+05 5,27E+03 1,43E+04 6,95E+04 4,34E+02 -2,92E+05
HTP-c1 CTUh 1,83E-05 0,00E+00 1,56E-07 2,90E-05 5,89E-07 0,00E+00 4,02E-06 2,18E-08 -6,80E-06
HTP-nc1 CTUh 4,61E-04 0,00E+00 3,73E-06 2,03E-04 4,85E-06 1,56E-05 8,72E-05 8,07E-07 -2,73E-04
SQP1 dimensionless 1,63E+05 1,62E+02 9,35E+02 5,86E+04 1,24E+03 1,35E+04 7,03E+03 6,26E+02 -2,72E+05
PM = Particulate Matter emissions; IRP = Ionizing radiation – human health; ETP-fw = Eco toxicity – freshwater; HTP-c = Human toxicity – cancer effects; HTP-nc =
Human toxicity – non cancer effects; SQP = Potential Soil Quality Index (dimensionless)
"Reading example: 9,0 E-03 = 9,0*10-3 = 0,009"
*INA Indicator Not Assessed
1. The results of this environmental impact indicator shall be used with care as the uncertainties on these results are high or as there is limited experienced with the
indicator
2. This impact category deals mainly with the eventual impact of low dose ionizing radiation on human health of the nuclear fuel cycle. It does not consider effects due
to possible nuclear accidents, occupational exposure nor due to radioactive waste disposal in underground facilities. Potential ionizing radiation from the soil, from
radon and from some construction materials is also not measured by this indicator.
7 / 11
Resource use
Indicator Unit A1 A2 A3 A4 C1 C2 C3 C4 D
PERE MJ 1,30E+05 8,14E+00 3,97E+01 2,00E+03 5,47E+01 2,76E+02 1,31E+04 1,38E+01 -2,47E+05
PERM MJ 3,46E+03 0,00E+00 0,00E+00 0,00E+00 0,00E+00 0,00E+00 0,00E+00 0,00E+00 0,00E+00
PERT MJ 1,34E+05 8,14E+00 3,97E+01 2,00E+03 5,47E+01 2,76E+02 1,31E+04 1,38E+01 -2,47E+05
PENRE MJ 1,04E+06 1,21E+03 7,31E+03 4,55E+05 9,31E+03 1,93E+04 4,34E+04 2,28E+02 -2,51E+05
PENRM MJ 1,06E+06 0,00E+00 0,00E+00 0,00E+00 0,00E+00 0,00E+00 -1,06E+06 0,00E+00 -1,72E+05
PENRT MJ 2,10E+06 1,21E+03 7,31E+03 4,55E+05 9,31E+03 1,93E+04 -1,02E+06 2,28E+02 -4,23E+05
SM kg 0,00E+00 0,00E+00 0,00E+00 0,00E+00 0,00E+00 0,00E+00 0,00E+00 0,00E+00 -1,27E+01
RSF MJ 3,06E+03 2,00E-01 9,79E-01 0,00E+00 0,00E+00 9,89E+00 3,50E+01 3,42E-01 -3,31E+02
NRSF MJ 6,52E+01 2,76E+00 1,44E+01 0,00E+00 0,00E+00 3,54E+01 0,00E+00 4,71E+01 -1,44E+04
FW m3 1,32E+03 6,28E-02 3,83E-01 1,82E+01 4,95E-01 2,06E+00 1,38E+02 2,10E-01 -4,30E+02
PERE = Use of renewable primary energy excluding renewable primary energy resources used as raw materials; PERM = Use of renewable primary energy resources used
as raw materials; PERT = Total use of renewable primary energy resources; PENRE = Use of non renewable primary energy excluding non-renewable primary energy
resources used as raw materials; PENRM = Use of non renewable primary energy resources used as raw materials; PENRT = Total use of non renewable primary energy
resources; SM = Use of secondary materials; RSF = Use of renewable secondary fuels; NRSF = Use of non-renewable secondary fuels; FW = Net use of fresh water
"Reading example: 9,0 E-03 = 9,0*10-3 = 0,009"
*INA Indicator Not Assessed
8 / 11
End of life - Waste
Indicator Unit A1 A2 A3 A4 C1 C2 C3 C4 D
HWD kg 1,39E+02 5,14E-02 5,37E-01 1,32E+01 3,36E-01 9,96E-01 6,41E+00 3,91E+02 -1,06E+01
NHWD kg 3,56E+03 2,80E+00 1,01E+01 5,95E+02 1,82E+01 9,39E+02 2,73E+02 2,16E+02 -1,30E+03
RWD kg 2,12E+00 8,40E-03 5,08E-02 3,23E+00 6,53E-02 1,32E-01 9,96E-02 1,37E-03 -3,77E-01
HWD = Hazardous waste disposed; NHWD = Non-hazardous waste disposed; RWD = Radioactive waste disposed
"Reading example: 9,0 E-03 = 9,0*10-3 = 0,009"
*INA Indicator Not Assessed
End of life - Output flow
Indicator Unit A1 A2 A3 A4 C1 C2 C3 C4 D
CRU kg 0,00E+00 0,00E+00 0,00E+00 0,00E+00 0,00E+00 0,00E+00 0,00E+00 0,00E+00 0,00E+00
MFR kg 0,00E+00 0,00E+00 1,81E+01 0,00E+00 0,00E+00 0,00E+00 9,12E+03 0,00E+00 -2,87E+00
MER kg 0,00E+00 0,00E+00 3,12E+01 0,00E+00 0,00E+00 0,00E+00 1,69E+04 0,00E+00 -1,13E+01
EEE MJ 0,00E+00 0,00E+00 2,17E+01 0,00E+00 0,00E+00 0,00E+00 3,12E+04 0,00E+00 -1,75E+01
EET MJ 0,00E+00 0,00E+00 3,28E+02 0,00E+00 0,00E+00 0,00E+00 4,73E+05 0,00E+00 -2,65E+02
CRU = Components for re-use; MFR = Materials for recycling; MER = Materials for energy recovery; EEE = Exported energy electrical; EET = Exported energy thermal
"Reading example: 9,0 E-03 = 9,0*10-3 = 0,009"
*INA Indicator Not Assessed
Biogenic Carbon Content
Indicator Unit At the factory gate
Biogenic carbon content in product kg C 0,00E+00
Biogenic carbon content in accompanying packaging kg C 2,07E+01
Note: 1 kg biogenic carbon is equivalent to 44/12 kg CO2
9 / 11
Additional requirements
Greenhouse gas emissions from the use of electricity in the manufacturing phase
National production mix from import, low voltage (production of transmission lines, in addition to direct emissions and losses in grid) of applied
electricity for the manufacturing process (A3).
Dangerous substances
The product contains no substances given by the REACH Candidate list.
Indoor environment
Additional Environmental Information
Additional environmental impact indicators required in NPCR Part A for construction products
Indicator Unit A1 A2 A3 A4 C1 C2 C3 C4 D
GWPIOBC kg CO2 -eq 6,32E+04 9,45E+01 5,31E+02 3,34E+04 6,86E+02 1,28E+03 5,07E+04 3,82E+01 -1,42E+04
GWP-IOBC: Global warming potential calculated according to the principle of instantaneous oxidation. In order to increase the transparency of biogenic carbon​
contribution to climate impact, the indicator GWP-IOBC is required as it declares climate impacts calculated according to the principle of instantaneous oxidation.​
GWP-IOBC is also referred to as GWP-GHG in context to Swedish public procurement legislation.
10 / 11
Bibliography
ISO 14025:2010. Environmental labels and declarations - Type III environmental declarations - Principles and procedures. International
Organization for Standardization.
ISO 14044:2006. Environmental management - Life cycle assessment - Requirements and guidelines. International Organization for
Standardization.
EN 15804:2012+A2:2019. Environmental product declaration - Core rules for the product category of construction products. European
Committee for Standardization.
ISO 21930:2017. Sustainability in buildings and civil engineering works - Core rules for environmental product declarations of construction
products. International Organization for Standardization.
Ecoinvent v3, 2019. Allocation, cut-off by classification. Swiss Centre of Life Cycle Inventories.
Iversen et al., (2021). eEPD v2021.09, background information for EPD generator tool system verification, LCA.no. Report number: 07.21. System
verification report.
Gaspard Philis (2023). EPD generator for NPCR 031 part B for aquaculture infrastructure and components, Background information for EPD
generator application and LCA data, LCA.no report number: 03.23. PCR verification report.
EPD Norway (2022). NPCR Part A: Construction products and services. The Norwegian EPD foundation. Version 2.0 published 24.03.2021.
EPD Norway (2023). NPCR 031 Part B for aquaculture infrastructure and components. The Norwegian EPD foundation. Version 1.0 published
26.04.2023.
Program operator and publisher Phone: +47 977 22 020
The Norwegian EPD Foundation e-mail: post@epd-norge.no
Post Box 5250 Majorstuen, 0303 Oslo, Norway web: www.epd-norge.no
Owner of the declaration: Phone: +4792032311
Mørenot Aquaculture AS e-mail: liv.lund@morenot.com
Langelandsvegen 35, 6010 Ålesund web: https://www.morenot.com/
Author of the Life Cycle Assessment Phone: +47 916 50 916
LCA.no AS e-mail: post@lca.no
Dokka 6A, 1671 web: www.lca.no
Developer of EPD generator Phone: +47 916 50 916
LCA.no AS e-mail: post@lca.no
Dokka 6B,1671 Kråkerøy web: www.lca.no
ECO Platform web: www.eco-platform.org
ECO Portal web: ECO Portal
11 / 11
