Environmental product declaration
in accordance with ISO 14025 and EN 15804+A2
Ready mixed concrete C35/45 SCC CEM I (XD1, XS1, XS2, XF2, XF3, XA2)
Owner of the declaration: Program operator:
A/S Ikast Betonvarefabrik The Norwegian EPD Foundation
Product: Declaration number:
Ready mixed concrete C35/45 SCC CEM I (XD1, XS1, XS2,
XF2, XF3, XA2) NEPD-8794-8456
Declared unit: Registration number:
1 m3
NEPD-8794-8456
This declaration is based on Product Category Rules:
Issue date: 23.01.2025
CEN Standard EN 15804:2012+A2:2019 serves as core
The Norwegian EPD Foundation PCR Valid to: 23.01.2030
EN 16757:2022 for Concrete and concrete elements
EPD software:
LCAno EPD generator ID: 747447
1 / 12
General information
Product Owner of the declaration:
Ready mixed concrete C35/45 SCC CEM I (XD1, XS1, XS2, XF2, XF3, A/S Ikast Betonvarefabrik
XA2) Contact person: Esben Mølgaard
Phone: +45 97152022
e-mail: ibf@ibf.dk
Program operator: Manufacturer:
The Norwegian EPD Foundation A/S Ikast Betonvarefabrik
Post Box 5250 Majorstuen, 0303 Oslo, Norway
Phone: +47 977 22 020
web: www.epd-norge.no
Declaration number: Place of production:
A/S Ikast Betonvarefabrik
NEPD-8794-8456
Lysholt Allé 4
7430 Ikast, Denmark
This declaration is based on Product Category Rules: Management system:
CEN Standard EN 15804:2012+A2:2019 serves as core PCR
EN 16757:2022 for Concrete and concrete elements
Statement of liability: Organisation no:
The owner of the declaration shall be liable for the underlying 37537314
information and evidence. EPD Norway shall not be liable with respect
to manufacturer information, life cycle assessment data and
evidences.​
Declared unit: Issue date:
1 m3 Ready mixed concrete C35/45 SCC CEM I (XD1, XS1, XS2, XF2, 23.01.2025
XF3, XA2)
Declared unit with option: Valid to:
A1,A2,A3,A4,C1,C2,C3,C4,D 23.01.2030
Year of study:
2024
Functional unit: Comparability:
- EPD of construction products may not be comparable if they not
comply with EN 15804 and seen in a building context.
General information on verification of EPD from EPD tools: Development and verification of EPD:
Independent verification of data, other environmental information The declaration is created using EPD tool lca.tools ver EPD2022.03,
and the declaration according to ISO 14025:2010, § 8.1.3 and § 8.1.4. developed by LCA.no. The EPD tool is integrated in the company's
Verification of each EPD is made according to EPD-Norway’s management system, and has been approved by EPD Norway.
guidelines for verification and approval requiring that tools are i)
integrated into the company's environmental management system, ii) Developer of EPD: Reza Wali
the procedures for use of the EPD tool are approved by EPD-Norway,
Reviewer of company-specific input data and EPD:​ Eva Brandt Larsen
and iii) the process is reviewed annually by an independent third
party verifier. See Appendix G of EPD-Norway's General Programme
Instructions for further information on EPD tools
Verification of EPD tool: Approved:
Independent third party verification of the EPD tool, background data
and test-EPD in accordance with EPDNorway's procedures and
guidelines for verification and approval of EPD tools.
Third party verifier:
Alexander Borg, Asplan Viak AS
(no signature required)
2 / 12
Product
Product description:
This specific product EPD covers:
Ready mixed concrete C35/45 SCC for aggressive environment with CEM I 52,5 (MS/LA) cement.
The EPD covers all consistency and Dmax variants of this specific concrete type, delivered from IBF production plants in Denmark.
Additions such as fibres and pigments are not included.
Raw materials is based on consumption from January 2024 to December 2024.
Product specification
For further information, see https.//www.ibf.dk/
Materials Value Unit
Ready mixed concrete 2266 kg/m3
Technical data:
The concrete are produced and delivered according to EN 206 and DS 206.
Strength class: C35/45
Exposure classes: XD1, XS1, XS2, XF2, XF3 and XA2
Slump-flow: 550-650 mm
Dmax: 8 mm, 16 mm and 32 mm
Market:
Denmark
Reference service life, product
Reference service lifetime, product is calculated as 100 years (RSL) cf. Annex AA in EN 16757:2017, Sustainability of construction works -
Environmental product declarations - Product Category Rules for concrete and concrete elements.
Reference service life, building or construction works
Reference service lifetime: the building is declarered as 50 years, as this is the chosen as the reference period for depreciation in Denmark.
LCA: Calculation rules
Declared unit:
1 m3 Ready mixed concrete C35/45 SCC CEM I (XD1, XS1, XS2, XF2, XF3, XA2)
Cut-off criteria:
All major raw materials and all the essential energy is included. The production processes for raw materials and energy flows with very small
amounts (less than 1%) are not included. These cut-off criteria do not apply for hazardous materials and substances.
Allocation:
The allocation is made in accordance with the provisions of EN 15804. Incoming energy and water and waste production in-house is allocated
equally among all products through mass allocation. Effects of primary production of recycled materials is allocated to the main product in which
the material was used. The recycling process and transportation of the material is allocated to this analysis.
Data quality:
Specific data for the product composition are provided by the manufacturer. The data represent the production of the declared product and were
collected for EPD development in the year of study. Background data is based on EPDs according to EN 15804 and different LCA databases. The
data quality of the raw materials in A1 is presented in the table below.
3 / 12
Materials Source Data quality Year
Aggregate ecoinvent 3.6 Database 2019
Aggregate Ref: NEPD-4799-4059-EN EPD 2020
Aggregate S-P-04034 EPD 2021
Cement S-P-06379 EPD 2020
Chemical EPD-EFC-20210193-IBG1-EN EPD 2021
Chemical EPD-EFC-20210194-IBG1-EN EPD 2021
Chemical EPD-EFC-20210195-IBG1-EN EPD 2021
Chemical EPD-EFC-20210197-IBG1-EN EPD 2021
Chemical EPD-EFC-20210198-IBG1-EN EPD 2021
Pigments and Fillers MD-20026-DA EPD 2020
Sand ecoinvent 3.6 Database 2019
Sand S-P-02081 EPD 2021
Water ecoinvent 3.6 Database 2019
Direct
Water EF v3.0 Characterization 2021
factors.
4 / 12
System boundaries (X=included, MND=module not declared, MNR=module not relevant)
Construction Beyond the system
Product stage Use stage End of life stage
installation stage boundaries
A1 A2 A3 A4 A5 B1 B2 B3 B4 B5 B6 B7 C1 C2 C3 C4 D
X X X X MND MND MND MND MND MND MND MND X X X X X
System boundary:
Additional technical information:
According to DS 206, concrete produced for exposure classes XD1, XS1, XS2, XF2, XF3 and XA2 can be used for:
Concrete surfaces exposed to airborne chlorides from de-icing agents, areas with limited de-icing, or surfaces close to areas being de-iced (XD1).
Concrete exposed to airborne salt from seawater (XS1). Concrete in permanent contact with seawater (XS2). Vertical concrete surfaces exposed to
freezing and airborne de-icing agents (XF2). Horizontal concrete surfaces exposed to rain and freezing (XF3). Concrete exposed to soil and
groundwater with a moderately aggressive chemical environment (XA2).
For informative examples see DS 206.
For further specifications, contact nearest IBF department: https://www.ibf.dk/professionel/Fabriksbeton/Kontakt/
waR slairetam tropsnarT gnirutcafunaM tropsnarT ylbmessA e​sU ecnanetniaM riapeR tnemecalpeR tnemhsibrufeR lanoitarepO ygrene esu lanoitarepO esu retaw -eD noitcurtsnoc noitilomed tropsnarT etsaW gnissecorp lasopsiD -yrevoceR-esueR laitnetop-gnilcyceR
5 / 12
LCA: Scenarios and additional technical information
The following information describe the scenarios in the different modules of the EPD.
Capacity utilisation Value
Transport from production place to user (A4) Distance (km) Fuel/Energy Consumption Unit
(incl. return) % (Liter/tonne)
Concrete truck, EURO 6 (km) - Europe 53,3 % 25 0,023 l/tkm 0,58
De-construction demolition (C1) Unit Value
Demolition of building per kg of cement-based
kg 2265,77
product, C1 (kg)
Capacity utilisation Value
Transport to waste processing (C2) Distance (km) Fuel/Energy Consumption Unit
(incl. return) % (Liter/tonne)
Truck, over 32 tonnes, EURO 6 (km) - Europe 53,3 % 25 0,023 l/tkm 0,58
Waste processing (C3) Unit Value
Waste treatment of cement-based product after
kg 2192,36
demolition, C3 (kg)
Disposal (C4) Unit Value
Waste, concrete, to landfill (kg) kg 73,41
Benefits and loads beyond the system
Unit Value
boundaries (D)
Substitution of primary aggregates, gravel round
kg 2192,36
(kg)
6 / 12
LCA: Results
The LCA results are presented below for the declared unit defined on page 2 of the EPD document.
Environmental impact
Indicator Unit A1 A2 A3 A4 C1 C2 C3 C4 D
GWP-total kg CO2 -eq 3,34E+02 1,94E+01 3,01E+00 4,94E+00 9,06E+00 4,94E+00 1,58E+00 3,15E-01 -5,12E+00
GWP-fossil kg CO2 -eq 3,33E+02 1,94E+01 2,98E+00 4,93E+00 9,06E+00 4,93E+00 1,56E+00 3,14E-01 -5,02E+00
GWP-biogenic kg CO2 -eq 1,09E+00 6,42E-03 2,96E-02 2,11E-03 1,70E-03 2,11E-03 1,34E-02 2,67E-04 -1,00E-01
GWP-luluc kg CO2 -eq 1,04E-01 4,87E-03 3,69E-03 1,50E-03 7,15E-04 1,50E-03 2,15E-03 6,17E-05 -3,39E-03
ODP kg CFC11 -eq 5,64E-06 4,49E-06 3,35E-07 1,19E-06 1,96E-06 1,19E-06 3,07E-07 1,53E-07 -9,14E-07
AP mol H+ -eq 9,15E-01 2,44E-01 1,74E-02 1,59E-02 9,48E-02 1,59E-02 1,26E-02 3,07E-03 -4,52E-02
EP-FreshWater kg P -eq 4,94E-03 1,13E-04 1,46E-04 3,93E-05 3,30E-05 3,93E-05 9,84E-05 2,35E-06 -1,33E-04
EP-Marine kg N -eq 1,49E-01 5,49E-02 5,54E-03 3,48E-03 4,19E-02 3,48E-03 3,69E-03 1,15E-03 -1,57E-02
EP-Terrestial mol N -eq 1,64E+00 6,13E-01 6,37E-02 3,88E-02 4,53E-01 3,88E-02 4,25E-02 1,27E-02 -1,84E-01
POCP kg NMVOC -eq 5,33E-01 1,71E-01 1,65E-02 1,52E-02 1,26E-01 1,52E-02 1,14E-02 3,63E-03 -4,86E-02
ADP-minerals&metals1 kg Sb-eq 1,09E-03 2,38E-04 3,20E-05 8,79E-05 1,39E-05 8,79E-05 1,98E-05 2,78E-06 -4,46E-04
ADP-fossil1 MJ 1,27E+03 2,92E+02 4,20E+01 8,01E+01 1,25E+02 8,01E+01 4,83E+01 1,01E+01 -8,49E+01
WDP1 m3 2,66E+03 1,76E+02 3,61E+02 6,14E+01 2,65E+01 6,14E+01 5,34E+03 2,14E+01 -3,98E+03
GWP-total = Global Warming Potential total; GWP-fossil = Global Warming Potential fossil fuels; GWP-biogenic = Global Warming Potential biogenic; GWP-luluc =
Global Warming Potential land use and land use change; ODP = Depletion potential of the stratospheric ozone layer; AP = Acidification potential, Accumulated
Exceedance; EP-freshwater = Eutrophication potential, fraction of nutrients reaching freshwater end compartment: EP-marine = Eutrophication potential, fraction of
nutrients reaching marine end compartment; EP-terrestrial = Eutrophication potential, Accumulated Exceedance; POCP = Formation potential of tropospheric ozone;
ADP-minerals&metals = Abiotic depletion potential for non-fossil resources; ADP-fossil = Abiotic depletion for fossil resources potential; WDP = Water (user)
deprivation potential, deprivation-weighted water consumption
"Reading example: 9,0 E-03 = 9,0*10-3 = 0,009"
*INA Indicator Not Assessed
1. The results of this environmental impact indicator shall be used with care as the uncertainties on these results are high or as there is limited experienced with the
indicator
Remarks to environmental impacts
7 / 12
Additional environmental impact indicators
Indicator Unit A1 A2 A3 A4 C1 C2 C3 C4 D
PM Disease incidence 9,65E-06 1,37E-06 3,94E-07 4,53E-07 1,15E-05 4,53E-07 2,02E-07 6,53E-08 -9,62E-07
IRP2 kgBq U235 -eq 2,63E+00 1,28E+00 1,80E-01 3,50E-01 5,44E-01 3,50E-01 8,11E-01 4,40E-02 -7,79E-01
ETP-fw1 CTUe 2,85E+03 1,92E+02 7,03E+01 5,86E+01 6,82E+01 5,86E+01 3,43E+01 5,02E+00 -8,74E+01
HTP-c1 CTUh 2,35E-07 0,00E+00 2,13E-09 0,00E+00 2,27E-09 0,00E+00 2,19E-09 1,47E-10 -4,39E-09
HTP-nc1 CTUh 1,16E-06 1,46E-07 4,32E-08 5,66E-08 6,34E-08 5,66E-08 3,07E-08 2,94E-09 -1,07E-07
SQP1 dimensionless 8,72E+01 2,47E+02 7,80E+01 9,19E+01 1,52E+01 9,19E+01 2,73E+01 3,70E+01 1,93E+02
PM = Particulate Matter emissions; IRP = Ionizing radiation – human health; ETP-fw = Eco toxicity – freshwater; HTP-c = Human toxicity – cancer effects; HTP-nc =
Human toxicity – non cancer effects; SQP = Potential Soil Quality Index (dimensionless)
"Reading example: 9,0 E-03 = 9,0*10-3 = 0,009"
*INA Indicator Not Assessed
1. The results of this environmental impact indicator shall be used with care as the uncertainties on these results are high or as there is limited experienced with the
indicator
2. This impact category deals mainly with the eventual impact of low dose ionizing radiation on human health of the nuclear fuel cycle. It does not consider effects due
to possible nuclear accidents, occupational exposure nor due to radioactive waste disposal in underground facilities. Potential ionizing radiation from the soil, from
radon and from some construction materials is also not measured by this indicator.
8 / 12
Resource use
Indicator Unit A1 A2 A3 A4 C1 C2 C3 C4 D
PERE MJ 1,98E+02 2,89E+00 2,67E+01 1,01E+00 6,80E-01 1,01E+00 2,49E+01 1,56E-01 -1,99E+01
PERM MJ 1,18E-04 0,00E+00 0,00E+00 0,00E+00 0,00E+00 0,00E+00 0,00E+00 0,00E+00 0,00E+00
PERT MJ 1,98E+02 2,89E+00 2,67E+01 1,01E+00 6,80E-01 1,01E+00 2,49E+01 1,56E-01 -1,99E+01
PENRE MJ 1,25E+03 2,92E+02 4,20E+01 8,01E+01 1,25E+02 8,01E+01 4,84E+01 1,01E+01 -8,96E+01
PENRM MJ 2,74E+01 0,00E+00 0,00E+00 0,00E+00 0,00E+00 0,00E+00 0,00E+00 0,00E+00 0,00E+00
PENRT MJ 1,28E+03 2,92E+02 4,20E+01 8,01E+01 1,25E+02 8,01E+01 4,84E+01 1,01E+01 -8,96E+01
SM kg 2,01E-02 0,00E+00 2,05E-04 0,00E+00 0,00E+00 0,00E+00 0,00E+00 0,00E+00 0,00E+00
RSF MJ 2,79E-01 1,05E-01 6,37E-01 3,53E-02 0,00E+00 3,53E-02 0,00E+00 3,23E-03 -4,07E-01
NRSF MJ 3,15E-01 3,53E-01 3,36E-02 1,18E-01 0,00E+00 1,18E-01 0,00E+00 9,28E-03 -4,18E-01
FW m3 2,22E+00 2,47E-02 1,19E-01 9,12E-03 6,42E-03 9,12E-03 8,28E-02 1,21E-02 -3,12E+00
PERE = Use of renewable primary energy excluding renewable primary energy resources used as raw materials; PERM = Use of renewable primary energy resources used
as raw materials; PERT = Total use of renewable primary energy resources; PENRE = Use of non renewable primary energy excluding non-renewable primary energy
resources used as raw materials; PENRM = Use of non renewable primary energy resources used as raw materials; PENRT = Total use of non renewable primary energy
resources; SM = Use of secondary materials; RSF = Use of renewable secondary fuels; NRSF = Use of non-renewable secondary fuels; FW = Net use of fresh water
"Reading example: 9,0 E-03 = 9,0*10-3 = 0,009"
*INA Indicator Not Assessed
9 / 12
End of life - Waste
Indicator Unit A1 A2 A3 A4 C1 C2 C3 C4 D
HWD kg 8,67E+00 1,34E-02 4,08E-02 4,38E-03 3,67E-03 4,38E-03 4,83E-03 0,00E+00 -2,05E-02
NHWD kg 1,86E+02 1,80E+01 5,79E-01 6,97E+00 1,48E-01 6,97E+00 1,53E-01 7,34E+01 -6,21E-01
RWD kg 6,47E-03 2,02E-03 1,85E-04 5,47E-04 8,66E-04 5,47E-04 5,11E-04 0,00E+00 -6,74E-04
HWD = Hazardous waste disposed; NHWD = Non-hazardous waste disposed; RWD = Radioactive waste disposed
"Reading example: 9,0 E-03 = 9,0*10-3 = 0,009"
*INA Indicator Not Assessed
End of life - Output flow
Indicator Unit A1 A2 A3 A4 C1 C2 C3 C4 D
CRU kg 8,26E+00 0,00E+00 0,00E+00 0,00E+00 0,00E+00 0,00E+00 0,00E+00 0,00E+00 0,00E+00
MFR kg 1,74E+00 0,00E+00 2,95E+01 0,00E+00 0,00E+00 0,00E+00 2,19E+03 0,00E+00 0,00E+00
MER kg 8,90E-01 0,00E+00 1,32E-01 0,00E+00 0,00E+00 0,00E+00 0,00E+00 0,00E+00 0,00E+00
EEE MJ 0,00E+00 0,00E+00 7,79E-02 0,00E+00 0,00E+00 0,00E+00 0,00E+00 0,00E+00 0,00E+00
EET MJ 0,00E+00 0,00E+00 1,18E+00 0,00E+00 0,00E+00 0,00E+00 0,00E+00 0,00E+00 0,00E+00
CRU = Components for re-use; MFR = Materials for recycling; MER = Materials for energy recovery; EEE = Exported energy electrical; EET = Exported energy thermal
"Reading example: 9,0 E-03 = 9,0*10-3 = 0,009"
*INA Indicator Not Assessed
Biogenic Carbon Content
Indicator Unit At the factory gate
Biogenic carbon content in product kg C 0,00E+00
Biogenic carbon content in accompanying packaging kg C 0,00E+00
Note: 1 kg biogenic carbon is equivalent to 44/12 kg CO2
10 / 12
Additional requirements
Greenhouse gas emissions from the use of electricity in the manufacturing phase
National production mix from import, low voltage (production of transmission lines, in addition to direct emissions and losses in grid) of applied
electricity for the manufacturing process (A3).
Electricity mix Source Amount Unit
Electricity, Denmark (kWh) ecoinvent 3.6 338,20 g CO2-eq/kWh
Electricity, Denmark, solar (kWh) ecoinvent 3.6 77,03 g CO2-eq/kWh
Dangerous substances
The product contains no substances given by the REACH Candidate list.
Indoor environment
Additional Environmental Information
Additional environmental impact indicators
Indicator Unit A1 A2 A3 A4 C1 C2 C3 C4 D
GWPIOBC kg CO2 -eq 3,33E+02 1,94E+01 3,59E+00 4,94E+00 9,06E+00 4,94E+00 1,56E+00 3,15E-01 -5,37E+00
GWP-IOBC: Global warming potential calculated according to the principle of instantaneous oxidation. In order to increase the transparency of biogenic carbon​
contribution to climate impact, the indicator GWP-IOBC is required as it declares climate impacts calculated according to the principle of instantaneous oxidation.​
GWP-IOBC is also referred to as GWP-GHG in context to Swedish public procurement legislation.
11 / 12
Bibliography
ISO 14025:2010 Environmental labels and declarations - Type III environmental declarations - Principles and procedures.
ISO 14044:2006 Environmental management - Life cycle assessment - Requirements and guidelines.
EN 15804:2012+A2:2019 Environmental product declaration - Core rules for the product category of construction products.
ISO 21930:2017 Sustainability in buildings and civil engineering works - Core rules for environmental product declarations of construction
products.
ecoinvent v3, Allocation, cut-off by classification, Swiss Centre of Life Cycle Inventories.
Iversen et al., (2021) eEPD v2021.09 Background information for EPD generator tool system verification, LCA.no Report number: 07.21
Graafland et al., (2024) EPD generator for concrete and concrete elements, EN 16757 Background information for EPD generator application and
LCA data, LCA.no report number: 01.24
NS-EN 16757:2022 for concrete and concrete elements, Ver. 1.0, 04.11.2022, Standard Norway.
Program operator and publisher Phone: +47 977 22 020
The Norwegian EPD Foundation e-mail: post@epd-norge.no
Post Box 5250 Majorstuen, 0303 Oslo, Norway web: www.epd-norge.no
Owner of the declaration: Phone: +45 97152022
A/S Ikast Betonvarefabrik e-mail: ibf@ibf.dk
Lysholt Allé 4, 7430 Ikast, Denmark web: www.ibf.dk
Author of the Life Cycle Assessment Phone: +47 916 50 916
LCA.no AS e-mail: post@lca.no
Dokka 6A, 1671 Kråkerøy, Norway web: www.lca.no
Developer of EPD generator Phone: +47 916 50 916
LCA.no AS e-mail: post@lca.no
Dokka 6A, 1671 Kråkerøy, Norway web: www.lca.no
ECO Platform web: www.eco-platform.org
ECO Portal web: ECO Portal
12 / 12
