ver1 2015
ENVIRONMENTAL PRODUCT DECLARATION
in accordance with ISO 14025, ISO 21930 and EN 15804
Owner of the declaration: Skanska Industrial Solutions AB
Program operator: The Norwegian EPD Foundation
Publisher: The Norwegian EPD Foundation
Declaration number: NEPD-2820-1517-EN
Registration number: NEPD-2820-1517-EN
ECO Platform reference number: -
Issue date: 31.05.2021
Valid to: 31.05.2026
ABT Skanska Grön AsfaltBio Zero. Gällivare, Luleå, Umeå, Sundsvall,
Borlänge och Södertälje asfaltverk.
Skanska Industrial Solutions AB
www.epd-norge.no
NEPD-2820-1517-EN ABT Skanska Grön AsfaltBio Zero. Gällivare, Luleå, Umeå, Sundsvall, Borlänge och Södertälje asfaltverk.
1 / 8
General information
Product: Owner of the declaration:
ABT Skanska Grön AsfaltBio Zero. Gällivare, Luleå, Umeå, Sundsvall, Borlänge och Skanska Industrial Solutions AB
Södertälje asfaltverk. Contact person: Henrik Sjöholm
Phone: +46 10-448 71 06
e-mail: Henrik.Sjoholm@Skanska.se
Program operator: Manufacturer:
Skanska Industrial Solutions AB
The Norwegian EPD Foundation
Pb. 5250 Majorstuen, 0303 Oslo
Phone: +47 23 08 80 00
e-mail: post@epd-norge.no
Declaration number: Place of production:
Skanska Industrial Solutions AB
NEPD-2820-1517-EN Warfvinges väg 25 112 74 Stockholm
Sweden
ECO Platform reference number: Management system:
ISO 14001, ISO 9001
This declaration is based on Product Category Rules: Organisation no:
556793-1638
CEN Standard EN 15804:2012+A1:2013 serves as core PCR
NPCR 025:2017 Part B for Asphalt
Statement of liability: Issue date: 31.05.2021
The owner of the declaration shall be liable for the underlying information and
evidence. EPD Norway shall not be liable with respect to manufacturer Valid to: 31.05.2026
information, life cycle assessment data and evidences.
Declared unit: Year of study:
1 tonne ABT Skanska Grön AsfaltBio Zero. Gällivare, Luleå, Umeå, Sundsvall, Borlänge
2020
och Södertälje asfaltverk.
Declared unit with option: Comparability:
EPD of construction products may not be comparable if they not comply with EN
A1,A2,A3,A4
15804 and seen in a building context.
Functional unit: Development and verification of EPD:
The declaration has been developed and verified using EPD tool lca.tools
ver EPD2020.11, developed by LCA.no AS. The EPD tool is integrated into
the company's environmental management system, and has been
approved by EPD-Norway
General information on verification of EPD from EPD tools:
Independent verification of data, other environmental information and Developer of EPD:
the declaration according to ISO 14025:2010, § 8.1.3 and § 8.1.4. Individual
third party verification of each EPD is not required when the EPD tool is i) Henrik Sjoholm
integrated into the company's environmental management system, ii) the
procedures for use of the EPD tool are approved by EPDNorway, and iii) Reviewer of company-specific input data and EPD:
the proccess is reviewed annualy. See Appendix G of EPD-Norway's
General Programme Instructions for further information on EPD tools. Nicklas Magnusson
Verification of EPD tool: Approved:
Independent third party verification of the EPD tool, background data
Sign
and test-EPD in accordance with EPDNorway's procedures and guidelines
for verification and approval of EPD tools.
Erik Svanes, Norsus AS
(no signature required) Håkon Hauan, CEO EPD-Norge
NEPD-2820-1517-EN ABT Skanska Grön AsfaltBio Zero. Gällivare, Luleå, Umeå, Sundsvall, Borlänge och Södertälje asfaltverk.
2 / 8
Product
Product description: Technical data:
Asphalt Wearing course for road contruction.
ABT wearing course according to Swedish road administration specification
Product specification TDOK 2013:0529.
ABT 160/220, 100/150 Market:
Sweden
Materials kg %
Reference service life, product
Aggregate 749,00 74,90
Bitumen 42,90 4,29 Depending on traffic, road design and climate conditions.
Amin, CAS Nr. 68910-93-0 0,10 0,01 Reference service life, construction works
Bitumen from reclaimed asphalt 10,00 1,00
Depending on traffic, road design and climate conditions.
Aggregates from reclaimed asphalt 190,00 19,00
Biobased binder 8,00 0,80
Total: 1000,00
LCA: Calculation rules
Declared unit: Allocation:
1 tonne ABT Skanska Grön AsfaltBio Zero. Gällivare, Luleå, Umeå, The allocation is made in accordance with the provisions of EN 15804.
Sundsvall, Borlänge och Södertälje asfaltverk. Incoming energy and water and waste production in-house is allocated
equally among all products through mass allocation. Effects of primary
Cut-off criteria:
production of recycled materials is allocated to the main product in which
All major raw materials and all the essential energy is included. The the material was used. The recycling process and transportation of the
production processes for raw materials and energy flows with very small material is allocated to the analysis in this EPD. For bitumen production,
amounts (less than 1%) are not included. These cut-off criteria do not crude oil extraction and transport are allocated by mass, while the final
apply for hazardous materials and substances. products from oil refineries are allocated by economic factors.
Data quality:
Specific data for the product composition are provided by the manufacturer. They represent the production of the declared product and were collected for
EPD development in the year of study. Background data is based on registered EPDs according to EN 15804, Ostfold Research databases, ecoinvent and other
LCA databases. The data quality of the raw materials in A1 is presented in the table below.
Specific environmental data from EPDs (Skanska EPD), in accordance with EN 15804, have been used for aggregates. Similarly, specific data have been used
for transport distances from supplier to asphalt plant and for energy use at factory. Other data (e.g. waste) are estimated. Specific data from the supplier have
also been used for bio-based binder. For all other data, generic data available in EPD tool v4.0 have been used. Transport of reclaimed asphelt from the road
to asphalt factory includes a return distance.
For bitumen, generic data from Eurobitume is used because specific data cannot be determined from the mix of bitumen suppliers according to EU
standards etc. used by Skanska.
Environmental impact for reclaimed asphalt falls to previous product systems until arrival at the asphalt plant. The asphalt plant uses electricity marked "Good
Environmental Choice".
Materials Source Data quality Year
Aggregate NEPD-1257-403 EPD 2016
Aggregates from reclaimed asphalt Østfoldforskning Database 2017
Bitumen from reclaimed asphalt Østfoldforskning Database 2017
Bitumen Eurobitume LCI report 2019
Amin, CAS Nr. 68910-93-0 Supplier Eco footprint 2020
Biobased binder Supplier LCA Report 2020
NEPD-2820-1517-EN ABT Skanska Grön AsfaltBio Zero. Gällivare, Luleå, Umeå, Sundsvall, Borlänge och Södertälje asfaltverk.
3 / 8
System boundary:
Additional technical information:
Bio-based binder contains biogenic carbon equlvalvent to 23 kg CO2-e per tonne asphalt. At the end-of-life stage, the asphalt material is milled and recycled
into new asphalt mixes. Hence, the biogenic carbon serve as a long-term carbon sink. If considering the long term biogenic sink as negative to GHG-
emissions from A1-A3, the net sum is 0,7 kg CO2-e per tonne asphalt.
20% reclaimed asphalt is included.
100 % renewable fuel is used in production (A3).
NEPD-2820-1517-EN ABT Skanska Grön AsfaltBio Zero. Gällivare, Luleå, Umeå, Sundsvall, Borlänge och Södertälje asfaltverk.
4 / 8
LCA: Scenarios and additional technical information
The following information describe the scenarios in the different modules of the EPD.
Transport from production place to user (A4)
Capacity utilisation Fuel/Energy
Type Type of vehicle Distance km Unit Value (l/t)
(incl. return) % consumption
Truck 50,0 % Asfaltbil med henger, EURO 6 50 0,023668 l/tkm 1,18
Railway l/tkm
Boat l/tkm
Other Transportation l/tkm
NEPD-2820-1517-EN ABT Skanska Grön AsfaltBio Zero. Gällivare, Luleå, Umeå, Sundsvall, Borlänge och Södertälje asfaltverk.
5 / 8
LCA: Results
The LCA results are presented below for the declared unit defined on page 2 of the EPD document.
System boundaries (X=included, MND=module not declared, MNR=module not relevant)
Construction Beyond the
Product stage installation User stage End of life stage . system
stage bondaries
A1 A2 A3 A4 A5 B1 B2 B3 B4 B5 B6 B7 C1 C2 C3 C4 . D
X X X X MND MND MND MND MND MND MND MND MND MND MND MND . MND
Environmental impact
Parameter Unit A1-A3 A4
GWP kg CO 2 -eq 2,37E+01 4,34E+00
ODP kg CFC11 -eq 2,18E-06 9,00E-07
POCP kg C 2H 4-eq 1,32E-02 6,83E-04
AP kg SO 2 -eq 2,08E-01 1,13E-02
EP kg PO 3- -eq 6,71E-02 1,55E-03
4
ADPM kg Sb -eq 3,56E-05 1,08E-05
ADPE MJ 2,14E+03 7,13E+01
GWP Global warming potential; ODP Depletion potential of the stratospheric ozone layer; POCP Formation potential of tropospheric photochemical oxidants;
AP Acidification potential of land and water; EP Eutrophication potential; ADPM Abiotic depletion potential for non fossil resources; ADPE Abiotic depletion
potential for fossil resources
"Reading example: 9,0 E-03 = 9,0*10-3 = 0,009"
*INA Indicator Not Assessed
Remarks to environmental impacts
The results for GWP exclude biogenic CO2 (IPCC 2007).
Bio-based binder contains biogenic carbon equlvalvent to 23 kg CO2-e per tonne asphalt. At the end-of-life stage, the asphalt material is milled and recycled into new asphalt
mixes. Hence, the biogenic carbon serve as a long-term carbon sink. If considering the long term biogenic sink as negative to GHG-emissions from A1-A3, the net sum is 0,7 kg
CO2-e per tonne asphalt.
waR slairetam tropsnarT gnirutcafunaM tropsnarT ylbmessA esU ecnanetniaM riapeR tnemecalpeR tnemhsibrufeR lanoitarepO ygrene esu lanoitarepO esu
retaw
-eD noitcurtsnoc noitilomed tropsnarT etsaW gnissecorp lasopsiD -yrevoceR-esueR -gnilcyceR laitnetop
NEPD-2820-1517-EN ABT Skanska Grön AsfaltBio Zero. Gällivare, Luleå, Umeå, Sundsvall, Borlänge och Södertälje asfaltverk.
6 / 8
Resource use
Parameter Unit A1-A3 A4
RPEE MJ 5,19E+01 1,30E+00
RPEM MJ 2,13E+00 0,00E+00
TPE MJ 5,40E+01 1,30E+00
NRPE MJ 5,18E+02 7,35E+01
NRPM MJ 2,17E+03 0,00E+00
TRPE MJ 2,24E+03 7,35E+01
SM kg 2,00E+02 0,00E+00
RSF MJ 2,57E+02 0,00E+00
NRSF MJ 0,00E+00 0,00E+00
W m3 6,73E+00 1,74E-02
RPEE Renewable primary energy resources used as energy carrier; RPEM Renewable primary energy resources used as raw materials; TPE Total use of renewable
primary energy resources; NRPE Non renewable primary energy resources used as energy carrier; NRPM Non renewable primary energy resources used as
materials; TRPE Total use of non renewable primary energy resources; SM Use of secondary materials; RSF Use of renewable secondary fuels; NRSF Use of non
renewable secondary fuels; W Use of net fresh water
"Reading example: 9,0 E-03 = 9,0*10-3 = 0,009"
*INA Indicator Not Assessed
End of life - Waste
Parameter Unit A1-A3 A4
HW kg 2,53E-03 3,97E-05
NHW kg 5,26E+00 6,71E+00
RW kg INA* INA*
HW Hazardous waste disposed; NHW Non hazardous waste disposed; RW Radioactive waste disposed
"Reading example: 9,0 E-03 = 9,0*10-3 = 0,009"
*INA Indicator Not Assessed
End of life - Output flow
Parameter Unit A1-A3 A4
CR kg 0,00E+00 0,00E+00
MR kg 3,00E-02 0,00E+00
MER kg 2,20E-01 0,00E+00
EEE MJ INA* INA*
ETE MJ INA* INA*
CR Components for reuse; MR Materials for recycling; MER Materials for energy recovery; EEE Exported electric energy; ETE Exported thermal energy
"Reading example: 9,0 E-03 = 9,0*10-3 = 0,009"
*INA Indicator Not Assessed
NEPD-2820-1517-EN ABT Skanska Grön AsfaltBio Zero. Gällivare, Luleå, Umeå, Sundsvall, Borlänge och Södertälje asfaltverk.
7 / 8
Additional Norwegian requirements
Greenhouse gas emissions from the use of electricity in the manufacturing phase
National production mix from import, low voltage (production of transmission lines, in addition to direct emissions and losses in grid) of applied electricity for
the manufacturing process (A3).
Electricity mix Data source Amount Unit
El-mix, Sweden (kWh) ecoinvent 3.4 Alloc Rec 42,67 g CO2-ekv/kWh
Dangerous substances
The product contains no substances given by the REACH Candidate list or the Norwegian priority list.
Indoor environment
Bibliography
ISO 14025:2010 Environmental labels and declarations - Type III environmental declarations - Principles and procedures.
ISO 14044:2006 Environmental management - Life cycle assessment - Requirements and guidelines.
EN 15804:2012+A1:2013 Environmental product declaration - Core rules for the product category of construction products.
ISO 21930:2017 Sustainability in buildings and civil engineering works, Core rules for environmental product declarations of construction products.
ecoinvent v3, Alloc Rec, Swiss Centre of Life Cycle Inventories.
Iversen et al., (2018) eEPD v3.0 – Background information for EPD generator system, LCA.no report number 04.18.
Iversen et al., (2017) EPD generator for Asfalt, Bakgrunnsrapport for applikasjon og datagrunnlag, OR 11.17, Østfoldforskning.
NPCR Part A: Construction products and services. Ver. 1.0. April 2017, EPD-Norge.
NPCR Part B for Asphalt. NPCR 025 Ver. 1.1. December 2017, EPD-Norge.
Inventory report, LCA-inventeringsrapport EPD-Asfalt ABT-, AG- och ABb BioZero från Södertälje, Borlänge, Umeå, Luleå, Gällivare och Sundsvall asfaltverk.
Inventory report, LCA- inventeringsrapport EPD asfalt ABT 16 Vällsta 2020.
Program operator and publisher Phone: +47 23 08 80 00
The Norwegian EPD Foundation e-mail: post@epd-norge.no
Post Box 5250 Majorstuen, 0303 Oslo,Norway web: www.epd-norge.no
Owner of the declaration Phone: +46 10-448 71 06
Skanska Industrial Solutions AB e-mail: Henrik.Sjoholm@Skanska.se
Warfvinges väg 25 112 74 Stockholm web: www.skanska.se
Author of the Life Cycle Assessment Phone: +47 69 35 11 00
Østfoldforskning AS e-mail: post@ostfoldforskning.no
Stadion 4 1671 Kråkerøy web: www.ostfoldforskning.no
Developer of EPD generator Phone: +47 916 50 916
LCA.no AS e-mail: post@lca.no
Dokka 1C,1671 Kråkerøy web: www.lca.no
NEPD-2820-1517-EN ABT Skanska Grön AsfaltBio Zero. Gällivare, Luleå, Umeå, Sundsvall, Borlänge och Södertälje asfaltverk.
8 / 8
