Environmental Product
Declaration
In accordance with ISO 14025 and EN 15804 +A2
½
Owner of the declaration: Rockfon Product Name
(part of ROCKWOOL Group)
Rockfon® Chicago
Program holder and publisher:
The Norwegian EPD foundation MetallicTM grids
Declaration number: Metal grid load bearing system
for Rockfon ceiling tiles.
NEPD-3343-1979-EN
Registration Number:
Manufacturer
Rockfon, part of ROCKWOOL
NEPD-3343-1979-EN
Issue date: Group
Valid to:
23.03.2022
The Norwegian 23.03.2027
EPD Foundation ver-141024
ver-210223
ver-210223
General information
Product: Owner of the declaration:
Chicago Metallic™ Grids Rockfon (part of ROCKWOOL Group)
ROCKWOOL A/S, Hovedgaden 501D, 2640
Program Operator:
Hedehusene
The Norwegian EPD Foundation
Post Box 5250 Majorstuen, 0303 Oslo, Norway Contact person:
Tlf: +47 23 08 80 00 Phone:
Marc Navatier
e-mail: post@epd-norge.no e-mail:
+45 6194 6424
sustainability@rockfon.com
Decleration Number: Manufacturer:
Rockfon, part of ROCKWOOL Group
NEPD-3343-1979-EN
This declaration is based on Product
Rockwool Belgium nv
Category Rules:
CEN Standard EN 15804+A2 serves as core PCR
Place of production:
NPCR 013:2021, Part B for Steel and Aluminium
Oud Sluisstraat 5, 2110 Wijnegem, Belgium
Construction Products
Management system:
Statements:
ISO 14001, ISO 9001
The owner of the declaration shall be liable for the
underlying information and evidence. EPD
Organisation no:
Norway shall not be liable with respect to
78416513
manufacturer, life cycle assessment data and
evidences.
Issue date:
Declared unit:
1 kg of average Chicago Metallic™ metal grid
23.03.2022
system for ceiling tiles. Valid to:
Declared unit with option:
23.03.2027
- Year of study:
2021
Functional unit:
Not applicable Comparability:
EPD of construction products may not be
Verification:
comparable if they not comply with EN
Independent verification of the declaration and
15804+A2 and seen in a building context.
data, according to ISO14025:2010
internal external LTahreis aE XPaDn thhaosp obueleonu, w o rked out by:
ROCKWOOL International A/S
Jane Anderson, ConstructionLCA Ltd
Independent verifier approved by EPD Norway
Approved (Manager of EPD Norway)
EPD for the best environmental decision 2
ver-210223
Product
Product description:
Rockfon® Chicago MetallicTM grids are a metal grid system is installed on the ceiling for a load
bearing of ceiling tiles. The system consists of different components e.g. main runners, cross
tees, etc. varying in length and height. Screws or other accessories such as clips, used to support
the systems, are not provided together with the metal grids (as support accessories are not
produced by Rockfon) and therefore are not part of this EPD.
Product specification:
Rockfon® Chicago MetallicTM grids area product made from cold rolled galvanised steel and from
coated steel with average recycled content of 17,5 %.
Product materials (per 1 kg of average system) kg %
Hot dip galvanised steel 0,73 73
Galvanised pre-painted (coated) steel 0,27 27
Packaging materials kg %
Cardboard 0,0396 58,5
Plastic 0,0003 0,4
Wood 0,0278 41,1
Technical data:
All the Rockfon® Chicago MetallicTM grids system components have been assessed according the
suspended ceiling harmonized standard: EN 13964:2014 Suspended ceilings - Requirements
and test methods. The technical properties based on this standard are given in Table
Property Value Ref. Standard
depending on the exact
product. For product
Reaction to Fire A1 / A2-s1,d0 EN 13964:2014
specific information
please see the DoP.
relevant for T15- T24 -
T35 mainrunner and
cross tees, Ultraline,
Load Bearing capacity Monolithic, bandraster,
Admissible banding 15 Nm ≤ Adm M ≤ 750 Nm I-profiles and Z-profiles
EN 13964:2014
moment -big variation
Adm M (Nm) depending on the exact
product. For product
specific information
please see the DoP.
relevant for L, W, J, F
and C profiles - big
Load Bearing capacity variation depending on
EN 13964:2014
Admissible load 180 N ≤ Adm F ≤ 400 N the exact product. For
Adm F (N) product specific
information please see
the DoP.
depending on the exact
product. For product EN 13964:2014
Durability Class B-C-D
specific information
please see the DoP.
EPD for the best environmental decision 3
ver-210223
Market:
The Rockfon® Chicago MetallicTM grids are supplied to Rockfon customers in Europe and Asia and
in other export markets, excluding North America.
Reference service life, product:
Rockfon® Chicago MetallicTM grids are durable products and provide performance for a lifetime
of the building. For the purpose of this EPD reference service life is considered 50 years, which
is a usual assumption for the lifetime the building where the system is installed. Rockfon®
Chicago MetallicTM gridsystem’s components do not have to be replaced in the 50-year scenario.
In practice, the life span will be longer than 50 years, assuming that the metal grids are only
replaced due to loss of performance or building demolition. Replacement of metal grids due to
replacement of ceiling tiles for aesthetics or interior design purposes is not accounted for.
Reference service life, building:
Reference service life of a building is considered to be 50 years.
LCA: Calculation rules
Declated unit:
The declared unit is 1 kg of average Rockfon® Chicago MetallicTM grids load bearing system for
ceiling tiles for a 50 years reference lifetime.
The impacts of the total installed metal grid system can be calculated by multiplying the results
of the EPD with the total weight of the installed system. A table with the different products
available in the portfolio and their respective weight per running meter is provided under
‘additional technical information’ section.
Data quality:
All data represents the applicable geography, time and technology for the specific and generic
data, generally assessed as good and very good. Primary data is collected from respective
production site in Belgium for the reference year 2020. Generic data is from GaBi database
(version 2021) with GaBi Software version 10.0.1.92 used for calculations. The raw materials
data is from reference year 2019 or 2020 according to the database documentation, while no
data is older than 5 years.
Allocation:
The allocation is made in accordance with the provisions of EN 15804. Production activities,
electricity and energy consumption and waste generation are allocated equally among all
products from the production site through mass allocation.
System boundary:
The LCA is a cradle-to-grave study, addressing all life cycle stages identified in the EN15804. All
major raw materials, energy, electricity use and waste are included for all life cycle modules, see
flowchart below. There are no environmental impacts at use stage.
EPD for the best environmental decision 4
ver-210223
Cut-off criteria:
All major raw materials and all the essential energy are included. The production process for
raw materials and energy flows that are included with very small amounts (<1% energy, mass,
impact) are not included. This cut-off rule does not apply for hazardous materials and
substances. Data sets are complete according to the system boundary within the limits set by
the criteria for the exclusion of inputs and outputs. All relevant data, all applied materials
according to the recipe and the energy used, originate from the production data and have been
considered within the inventory analysis.
LCA: Scenarios and additional technical information
The following information describe the scenarios in the different modules of the EPD.
Transport from production place to assembly/user (A4)
Capacity utilisation (incl. Type of Fuel/Energy value
Type Distance KM
return) % vehicle consumption (l/t)
Truck-
Diesel:
Truck, Euro 6 85 % trailer, 28- 810 km 13,93 l/t
0,0172 l/tkm
34 t
Ship
Ship 70 % 143 km Heavy fuel oil
container
The distance in A4 is calculated based on weighted average from the transport statistics of the
manufacturer in the reference year.
Assembly (A5)
Unit Value
Electricity consumption kWh 0,03 kWh/kg
Product loss kg < 1%
EPD for the best environmental decision 5
ver-210223
Rockfon® Chicago MetallicTM grids are easy to install, using known construction techniques. The
installation requires use of handheld tools, some of which are power tools that consume
electricity (e.g. electric drill). The packaging waste from installation site is assumed to be
treated according to average eropean statistics packaging waste treatment rates (Eurostat,
2019). Benefits from material recycling and energy recovery from incineration process of
plastic and wood packaging are reported under Module D.
Use stage (B1, B2, B3, B4, B5, B6, B7)
There are no consumables, maintenance, repair, replacements or refurbishments related to the
use of the metal grids for the period of the reference service life. Rockfon® Chicago MetallicTM
grids do not use energy or water during their operational life. There are no emissions released
from the product during the use. Replacement of the product due to aesthetic reasons (change
of interior design) and not related to the loss of performance is not taken into account.
Therefore, modules B1-B7 have zero impacts.
End of Life (C1, C3, C4)
Unit Value
kg 0
Hazardous waste disposed
kg 0
Collected as mixed construction waste
kg 0
Reuse
kg 0,98
Recycling
kg 0
Energy recovery
kg 0,02
To landfill
For steel, a 98% recovery rate is assumed, with 2% assumed to be landfilled. Reuse of metal
grids is not included in this scenario.
Transport to waste processing (C2)
Capacity utilisation (incl. Type of Fuel/Energy value
Type Distance KM
return) % vehicle consumption (l/t)
Truck-
Diesel:
Truck, Euro 6 50% trailer, 28- 100 km 2,95 l/t
0,03 l/tkm
34 t
The distance represents an average distance to the landfill or waste treatment facility.
Benefits and loads beyond the system boundaries (D)
Unit Value
Net scrap steel kg 0,81
Cardboard packaging kg 0,032
Plastic packaging kg 0,00024
Wood packaging kg 0,022
Quantities of packaging materials include both recycled materials and materials sent for energy
recovery.
EPD for the best environmental decision 6
ver-210223
Additional technical information
Below there is a list of all the products in Rockfon’s portfolio,together with their weight by
running meter. The weight of each product can be used to calculate the weight of the installed
system and to estimate the impacts of the entire system.
Average weight Average weight
Row Labels Row Labels
(kg/m) (kg/m)
Bandraster 100 mm 1,1 Main runner T15 Click / Hook 0,34
Bandraster 125 mm 1,4 Main runner T24 Click / Hook 0,39
Bandraster 150 mm 1,6 Monolithic furring channel 0,42
Bandraster 50 mm 0,8 Omega channel 50 mm 0,70
Bandraster 75 mm 1,0 Primary C-channel 12x38x12 mm 0,42
C-bandraster main runner 100 mm 1,1 Primary I-runner 0,78
Cross tee T15 Click / Hook 0,3 Screenline profile 0,34
Cross tee T24 Click / Hook 0,33 Spacer bars 0,17
C-section 15x11x13 mm 0,14 Spanfast™ main runner 0,52
C-wall angle 20x40x20 mm 0,33 Stepped Z-section 19 mm 0,20
F Profile 0,4 T24 x 75 mm system 0,77
Galvanised C-wall angle 30x40.5x30 mm 0,35 T35 system 0,46
I-runner 50 mm 2,42 Ultraline 0,35
J-wall angle 0,26 W-wall angle 0,35
L-wall angle 0,37 Z-section 0,40
T35x75 mm system 0,80
System boundaries (X=included, MND= module not declared, MNR=module not
relevant)
Benefits
& loads
Assembly
Product stage Use stage End of life stage beyond
stage
system
boundary
EPD for the best environmental decision 7
slairetam
waR
tropsnarT
gnirutcafunaM
tropsnarT ylbmessA
esU
ecnanetniaM
riapeR
tnemecalpeR tnemhsibrufeR
esu
ygrene
lanoitarepO
esu
retaw
lanoitarepO
noitilomed
noitcurtsnoc-eD
tropsnarT
gnissecorp
etsaW
lasopsiD
-gnilcyceR-yrevoceR-esueR
laitnetop
LCA: Results
A1 A2 A3 A4 A5 B1 B2 B3 B4 B5 B6 B7 C1 C2 C3 C4 D
X X X X X X X X X X X X X X X X X
The results are calculated based on declared unit of 1 kg of average Rockfon® Chicago MetallicTM
grid system. The impacts of the total installed metal grid system can be calculated by
multiplying the results of the EPD with the total weight of the installed system.
ver-210223
Core environmental impact indicators
Indicator Unit A1-A3 A4 A5 B* C1 C2 C3 C4 D
kg CO2
GWP-total 2,94E+00 4,34E-02 5,22E-02 0 1,20E-02 8,95E-03 0 9,78E-04 -1,37E+00
eq.
kg CO2
GWP-fossil 2,98E+00 4,29E-02 1,35E-02 0 1,19E-02 8,88E-03 0 9,77E-04 -1,40E+00
eq.
GWP- kg CO2
-3,99E-02 1,36E-04 3,87E-02 0 9,29E-05 0,00E+00 0 0,00E+00 2,97E-02
biogenic eq.
GWP- kg CO2
8,26E-04 3,44E-04 2,01E-05 0 2,00E-05 7,30E-05 0 9,77E-07 1,49E-04
LULUC eq.
kg
ODP CFC11 9,20E-13 8,42E-18 8,79E-12 0 2,90E-16 1,14E-18 0 2,31E-18 -6,37E-15
eq.
mol H⁺
AP 9,57E-03 8,05E-05 3,37E-05 0 2,16E-05 8,86E-06 0 3,11E-06 -2,54E-03
eq.
EP- kg P
1,89E-06 1,25E-07 1,14E-07 0 3,81E-08 2,65E-08 0 7,43E-10 -4,95E-07
freshwater eq.
kg N
EP-marine 2,16E-03 2,28E-05 1,25E-05 0 5,79E-06 2,83E-06 0 7,72E-07 -3,97E-04
eq.
EP- mol N
2,30E-02 2,62E-04 9,79E-05 0 6,06E-05 3,38E-05 0 8,47E-06 -3,90E-03
terrestial eq.
kg
POCP NMVO 7,14E-03 6,37E-05 3,14E-05 0 1,53E-05 7,70E-06 0 2,43E-06 -1,97E-03
C eq.
kg Sb
ADP-M&M 1,60E-05 3,76E-09 3,56E-09 0 3,71E-09 6,78E-10 0 6,74E-11 -3,01E-06
eq.
ADP-fossil MJ 3,09E+01 5,73E-01 2,31E-01 0 2,21E-01 1,19E-01 0 1,42E-02 -1,23E+01
WDP m³ 1,21E+00 3,92E-04 3,75E-03 0 1,80E-03 7,74E-05 0 -1,16E-05 -2,73E-01
GWP-total: Global Warming Potential; GWP-fossil: Global Warming Potential fossil fuels; GWP-biogenic:
Global Warming Potential biogenic; GWP-LULUC: Global Warming Potential land use and land use change;
ODP: Depletion potential of the stratospheric ozone layer; AP: Acidification potential, Accumulated
Exceedance; EP-freshwater: Eutrophication potential, fraction of nutrients reaching freshwater end
compartment; See “additional Norwegian requirements” for indicator given as PO4 eq. EP-marine:
Eutrophication potential, fraction of nutrients reaching freshwater end compartment; EP-terrestial:
Eutrophication potential, Accumulated Exceedance; POCP: Formation potential of tropospheric ozone; ADP-
M&M: Abiotic depletion potential for non-fossil resources (minerals and metals); ADP-fossil: Abiotic
depletion potential for fossil resources; WDP: Water deprivation potential, deprivation weighted water
counsumption.
Reading example: 9,0 E-03 = 9,0*10-3 = 0,009.
*There is no activity in any of the B modules, as described under the Use Stage previously. All the B modules are zero,
thus the result is presented in a single column B in all the tables.
EPD for the best environmental decision 8
ver-210223
Additional environmental impact indicators
Indicator Unit A1-A3 A4 A5 B C1 C2 C3 C4 D
Disease
PM 1,42E-07 9,37E-10 2,79E-10 0 1,79E-10 5,25E-11 0 3,37E-11 -4,68E-08
inc.
kBq
IRP U235 5,81E-02 1,51E-04 5,10E-03 0 3,05E-03 2,06E-05 0 2,32E-05 3,38E-02
eq.
ETP-fw CTUe 5,87E+00 4,25E-01 1,11E-01 0 8,53E-02 8,57E-02 0 4,18E-03 -8,22E-02
HTP-c CTUh 1,03E-09 8,58E-12 3,30E-12 0 2,71E-12 1,73E-12 0 4,86E-13 4,64E-10
HTP-nc CTUh 8,67E-08 4,44E-10 1,85E-10 0 9,61E-11 8,97E-11 0 4,88E-11 -1,90E-08
Dimen-
SQP 1,05E+01 1,93E-01 6,89E-02 0 8,37E-02 4,07E-02 0 1,05E-03 -4,94E+00
sionless
PM: Particulate matter emissions; IRP: Ionising radiation, human health; ETP-fw: Ecotoxicity (freshwater);
HTP-c: Human toxicity, cancer effects; HTP-nc: Human toxicity, non-cancer effects; SQP: Land use related
impacts / soil quality.
Classification of disclaimers to the declaration of core and additional environmental
impact indicators
ILCD
Indicator Disclaimer
classification
Global warming potential (GWP) None
ILCD type / level
Depletion potential of the stratospheric ozone layer (ODP) None
1
Potential incidence of disease due to PM emissions (PM) None
Acidification potential, Accumulated Exceedance (AP) None
Eutrophication potential, Fraction of nutrients reaching freshwater end
None
compartment (EP-freshwater)
Eutrophication potential, Fraction of nutrients reaching marine end
None
ILCD type / level compartment (EP-marine)
2
Eutrophication potential, Accumulated Exceedance (EP-terrestrial) None
Formation potential of tropospheric ozone (POCP) None
Potential Human exposure efficiency relative to U235 (IRP) 1
Abiotic depletion potential for non-fossil resources (ADP-minerals&metals) 2
Abiotic depletion potential for fossil resources (ADP-fossil) 2
Water (user) deprivation potential, deprivation-weighted water consumption
2
(WDP)
ILCD type / level
Potential Comparative Toxic Unit for ecosystems (ETP-fw) 2
3
Potential Comparative Toxic Unit for humans (HTP-c) 2
Potential Comparative Toxic Unit for humans (HTP-nc) 2
Potential Soil quality index (SQP) 2
Disclaimer 1 – This impact category deals mainly with the eventual impact of low dose ionizing radiation on
human health of the nuclear fuel cycle. It does not consider effects due to
possible nuclear accidents, occupational exposure nor due to radioactive waste disposal in underground facilities.
Potential ionizing radiation from the soil, from radon and from some
construction materials is also not measured by this indicator.
Disclaimer 2 – The results of this environmental impact indicator shall be used with care as the uncertainties on
these results are high or as there is limited experienced with the indicator
EPD for the best environmental decision 9
ver-210223
Resource use
Parameter Unit A1-A3 A4 A5 B C1 C2 C3 C4 D
RPEE MJ 9,01E-01 3,23E-02 9,66E-01 0 1,00E-01 6,62E-03 0 1,03E-03 7,25E-01
RPEM MJ 1,17E+00 0,00E+00 -8,69E-01 0 0,00E+00 0,00E+00 0 0,00E+00 0,00E+00
TPE MJ 2,06E+00 3,23E-02 9,76E-02 0 1,00E-01 6,62E-03 0 1,03E-03 7,25E-01
NRPE MJ 3,09E+01 5,75E-01 2,43E-01 0 2,21E-01 1,19E-01 0 1,42E-02 -1,23E+01
NRPM MJ 1,54E-02 0,00E+00 -1,16E-02 0 0,00E+00 0,00E+00 0 0,00E+00 0,00E+00
TRPE MJ 3,09E+01 5,75E-01 2,31E-01 0 2,21E-01 1,19E-01 0 1,42E-02 -1,23E+01
SM kg 1,75E-01 0,00E+00 0,00E+00 0 0,00E+00 0,00E+00 0 0,00E+00 0,00E+00
RSF MJ 0,00E+00 0,00E+00 0,00E+00 0 0,00E+00 0,00E+00 0 0,00E+00 0,00E+00
NRSF MJ 0,00E+00 0,00E+00 0,00E+00 0 0,00E+00 0,00E+00 0 0,00E+00 0,00E+00
W m3 3,01E-02 3,70E-05 1,38E-04 0 4,94E-05 7,58E-06 0 1,47E-07 -6,21E-03
RPEE Renewable primary energy resources used as energy carrier; RPEM Renewable primary energy
resources used as raw materials; TPE Total use of renewable primary energy resources; NRPE Non
renewable primary energy resources used as energy carrier; NRPM Non renewable primary energy
resources used as materials; TRPE Total use of non renewable primary energy resources; SM Use of
secondary materials; RSF Use of renewable secondary fuels; NRSF Use of non renewable secondary fuels; W
Use of net fresh water
End of life - Waste
Parameter Unit A1-A3 A4 A5 B C1 C2 C3 C4 D
HW kg 2,81E-08 2,98E-11 5,84E-11 0 6,59E-11 5,98E-12 0 2,52E-12 3,17E-09
NHW kg 1,55E-01 8,95E-05 9,67E-03 0 1,79E-04 1,76E-05 0 2,00E-02 1,45E-01
RW kg 1,87E-04 1,03E-06 3,13E-05 0 3,31E-05 1,44E-07 0 1,62E-07 -1,48E-05
HW Hazardous waste disposed; NHW Non hazardous waste disposed; RW Radioactive waste disposed
End of life – output flow
Parameter Unit A1-A3 A4 A5 B C1 C2 C3 C4 D
CR kg 0,00E+00 0,00E+00 0,00E+00 0 0,00E+00 0,00E+00 0 0,00E+00 0,00E+00
MR kg 7,77E-02 0,00E+00 4,41E-02 0 0,00E+00 9,80E-01 0 0,00E+00 0,00E+00
MER kg 0,00E+00 0,00E+00 0,00E+00 0 0,00E+00 0,00E+00 0 0,00E+00 0,00E+00
EEE MJ 2,42E-03 0,00E+00 2,75E-02 0 0,00E+00 0,00E+00 0 0,00E+00 0,00E+00
ETE MJ 5,55E-03 0,00E+00 4,83E-02 0 0,00E+00 0,00E+00 0 0,00E+00 0,00E+00
CR Components for reuse; MR Materials for recycling; MER Materials for energy recovery; EEE Exported
electric energy; ETE Exported thermal energy
Information describing the biogenic carbon content at the factory gate
Biogenic carbon content Unit Value
Biogenic carbon content in product kg C 0,00E+00
Biogenic carbon content in the accompanying packaging kg C 1,20E-02
EPD for the best environmental decision 10
ver-210223
Additional Norwegian requirements
Greenhouse gas emission from the use of electricity in the manufacturing phase
National production mix from import, low voltage (production of transmission lines, in addition
to direct emissions and losses in grid) of applied electricity for the manufacturing process(A3).
National electricity grid Unit Value
BG: Electricity grid mix (production mix), Sphera (GaBi) kg CO2 -eq/kWh 0,735
Additional environmental impact indicators required in NPCR Part A for construction
products
In order to increase the transparency of biogenic carbon contribution to climate impact, the
indicator for GWP has been sub-divided into the following:
GWP-IOBC Climate impacts calculated according to the principle of instantaneous oxidation
GWP-BC Climate impacts from the net uptake and emission of biogenic carbon from each
module.
In addition, EP-freshwater shall also declared as PO4 eq.
Indicator Unit A1-A3 A4 A5 B C1 C2 C3 C4 D
EP-
kg PO4 eq. 7,42E-04 5,49E-05 1,36E-05 0 2,67E-06 1,30E-06 0 2,71E-07 -1,20E-04
freshwater*
GWP-IOBC kg CO2 eq. 2,98E+00 4,34E-02 1,35E-02 0 1,19E-02 8,95E-03 0 9,78E-04 -1,40E+00
0,00E+0
GWP-BC kg CO2 eq. -3,99E-02 0,00E+00 3,87E-02 0 9,29E-05 0,00E+00 0 2,97E-02
0
GWP kg CO2 eq. 2,94E+00 4,34E-02 5,22E-02 0 1,20E-02 8,95E-03 0 9,78E-04 -1,37E+00
EP-freshwater* Eutrophication potential, fraction of nutrients reaching freshwater end compartment.
Declared as PO4 eq. GWP-IOBC Global warming potential calculated according to the principle of
instantanious oxidation. GWP-BC Global warming potential from net uptake and emissions of biogenic carbon
from the materials in each module. GWP Global warming potential
Hazardous substances
The declaration is based upon reference to threshold values and/or test results and/or material
safety data sheets provided to EPD verifiers. Documentation available upon request to EPD
owner.
□ The product contains no substances given by the REACH Candidate list or the Norwegian
priority list.
□ The product contains substances given by the REACH Candidate list or the Norwegian
priority list that are less than 0,1 % by weight.
□ The product contain dangerous substances, more then 0,1% by weight, given by the
REACH Candidate List or the Norwegian Priority list, see table.
□ The product contains no substances given by the REACH Candidate list or the Norwegian
priority list. The product is classified as hazardous waste (Avfallsforskiften, Annex III),
see table.
Indoor environment
Not relevant for this product category.
EPD for the best environmental decision 11
ver-210223
Carbon footprint
Carbon footprint of the 1 kg of Rockfon® Chicago MetallicTM grid system is 3,06 kg CO2 eq
(including Module A1-C4). This is elaborabed per module in the results section.
Additionally, carbon footprint estimated according to EN15804+A1, is 2,94 kg CO2 eq (Module
A1-C4). The results are elaborated in the Additional Results acc. EN15804+A1.
EPD for the best environmental decision 12
ver-210223
Additional LCA Results according to EN 15804+A1
Results in this section communicate LCA results developed for this EPD in the format described
in EN15804+A1:2013, in order to accommodate a need in the transition period between the two
standard revisions.
Environmental impacts
Indicator Unit A1-A3 A4 A5 B C1 C2 C3 C4 D
GWP kg CO2-eq. 2,83E+00 4,34E-02 4,55E-02 0 1,18E-02 8,73E-03 0 9,14E-04 -1,30E+00
kg CFC11-
ODP 1,23E-12 1,31E-17 1,15E-11 0 3,86E-16 1,52E-18 0 3,08E-18 -8,50E-15
eq.
AP kg SO2-eq. 7,84E-03 4,90E-04 2,64E-05 0 1,70E-05 6,50E-06 0 2,49E-06 -2,17E-03
kg PO43--
EP 7,42E-04 5,49E-05 1,36E-05 0 2,67E-06 1,30E-06 0 2,71E-07 -1,20E-04
eq.
kg ethene-
POCP 1,10E-03 2,48E-05 6,34E-06 0 1,51E-06 -1,47E-07 0 2,30E-07 -6,63E-04
eq.
ADPE kg Sb-eq. 1,57E-05 4,19E-09 3,47E-09 0 3,92E-09 6,79E-10 0 6,84E-11 -2,93E-06
ADPF MJ 2,89E+01 7,36E-01 1,51E-01 0 1,33E-01 1,18E-01 0 1,38E-02 -1,06E+01
GWP Global warming potential; ODP Depletion potential of the stratospheric ozone layer; POCP Formation
potential of tropospheric photochemical oxidants; AP Acidification potential of land and water; EP
Eutrophication potential; ADPM Abiotic depletion potential for non fossil resources; ADPE Abiotic depletion
potential for fossil resources.
Resource use
Parameter Unit A1-A3 A4 A5 B C1 C2 C3 C4 D
RPEE MJ 9,01E-01 3,23E-02 9,66E-01 0 1,00E-01 6,62E-03 0 1,03E-03 7,25E-01
0,00E+0
RPEM MJ 1,17E+00 0,00E+00 -8,69E-01 0 0,00E+00 0 0,00E+00 0,00E+00
0
TPE MJ 2,06E+00 3,23E-02 9,76E-02 0 1,00E-01 6,62E-03 0 1,03E-03 7,25E-01
NRPE MJ 3,09E+01 5,75E-01 2,43E-01 0 2,21E-01 1,19E-01 0 1,42E-02 -1,23E+01
0,00E+0
NRPM MJ 1,54E-02 0,00E+00 -1,16E-02 0 0,00E+00 0 0,00E+00 0,00E+00
0
TRPE MJ 3,09E+01 5,75E-01 2,31E-01 0 2,21E-01 1,19E-01 0 1,42E-02 -1,23E+01
0,00E+0
SM kg 1,75E-01 0,00E+00 0,00E+00 0 0,00E+00 0 0,00E+00 0,00E+00
0
0,00E+0
RSF MJ 0,00E+00 0,00E+00 0,00E+00 0 0,00E+00 0 0,00E+00 0,00E+00
0
0,00E+0
NRSF MJ 0,00E+00 0,00E+00 0,00E+00 0 0,00E+00 0 0,00E+00 0,00E+00
0
W m3 3,01E-02 3,70E-05 1,38E-04 0 4,94E-05 7,58E-06 0 1,47E-07 -6,21E-03
RPEE Renewable primary energy resources used as energy carrier; RPEM Renewable primary energy
resources used as raw materials; TPE Total use of renewable primary energy resources; NRPE Non
renewable primary energy resources used as energy carrier; NRPM Non renewable primary energy
resources used as materials; TRPE Total use of non renewable primary energy resources; SM Use of
secondary materials; RSF Use of renewable secondary fuels; NRSF Use of non renewable secondary fuels; W
Use of net fresh water.
EPD for the best environmental decision 13
ver-210223
End of life - Waste
Parameter Unit A1-A3 A4 A5 B C1 C2 C3 C4 D
HW kg 2,81E-08 2,98E-11 5,84E-11 0 6,59E-11 5,98E-12 0 2,52E-12 3,17E-09
NHW kg 1,55E-01 8,95E-05 9,67E-03 0 1,79E-04 1,76E-05 0 2,00E-02 1,45E-01
RW kg 1,87E-04 1,03E-06 3,13E-05 0 3,31E-05 1,44E-07 0 1,62E-07 -1,48E-05
HW Hazardous waste disposed; NHW Non hazardous waste disposed; RW Radioactive waste disposed.
End of life – output flow
Parameter Unit A1-A3 A4 A5 B C1 C2 C3 C4 D
0,00E+00 0,00E+00 0,00E+00 0,00E+00 0,00E+00 0,00E+00 0,00E+00
CR kg 0 0
7,77E-02 0,00E+00 4,41E-02 0,00E+00 9,80E-01 0,00E+00 0,00E+00
MR kg 0 0
0,00E+00 0,00E+00 0,00E+00 0,00E+00 0,00E+00 0,00E+00 0,00E+00
MER kg 0 0
2,42E-03 0,00E+00 2,75E-02 0,00E+00 0,00E+00 0,00E+00 0,00E+00
EEE MJ 0 0
5,55E-03 0,00E+00 4,83E-02 0,00E+00 0,00E+00 0,00E+00 0,00E+00
ETE MJ 0 0
CR Components for reuse; MR Materials for recycling; MER Materials for energy recovery; EEE Exported
electric energy; ETE Exported thermal energy.
EPD for the best environmental decision 14
ver-210223
Bibliography
ISO 14025:2010 Environmental labels and declarations - Type III environmental
declarations - Principles and procedures
ISO 14044:2006 Environmental management - Life cycle assessment -
Requirements and guidelines
EN 15804:2012+A2:2019 Sustainability of construction works - Environmental product
declaration - Core rules for the product category of construction
products
ISO 21930:2007 Sustainability in building construction - Environmental
declaration of building products
EPD-NORGE 2021 NPCR Part A:2021 Construction products and services. Reg
24.03.2021
EPD-NORGE 2021 NPCR 013:2021 Part B for Steel and aluminium construction
products. Reg 06.10.2021
ROCKWOOL Int. 2021 LCA report for Chicago Metallic™ (Rockfon) Grids for ceiling tiles
Program Operator tlf +47 23 08 80 00
The Norwegian EPD Foundation
Post Box 5250 Majorstuen, 0303 Oslo e-post: post@epd-norge.no
Norway web www.epd-norge.no
Publisher tlf +47 23 08 80 00
The Norwegian EPD Foundation
Post Box 5250 Majorstuen, 0303 Oslo e-post: post@epd-norge.no
Norway web www.epd-norge.no
Owner of the decleration tlf +45 52792930
Rockfon (part of ROCKWOOL Group)
Marc Navatier e-post:
web www.rockfon.com
Author of the life cycle assesment tlf +su4s5t a4i1n a5b0i l8it7y @51r ockfon.com
Larisa Xanthopoulou, LCA Specialist
ROCKWOOL Int. A/S
e-post: larisa.xanthopoulou@rockwool.com
Hovedgaden 584C, 2640 Hedehusene
Denmark web www.rockwool.com
EPD for the best environmental decision 15
ver-210223
EPD for the best
environmental
decision
The Norwegian EPD foundation
www.epd-norge.no
EPD for the best environmental decision 16
ver-210223
