Environmental product declaration
In accordance with ISO 14025 and EN 15804 +A2
Leca® 4-10 rund, Fibo ExClay Deutschland GmbH
Owner of the declaration: Program operator:
Leca International The Norwegian EPD Foundation
Declared unit: Declaration number:
1 m3 Leca® 4-10 rund, Fibo ExClay Deutschland GmbH
NEPD-3953-2890-EN
This declaration is based on Product Category Rules:
CEN Standard EN 15804:2012+A2:2019 serves as core PCR. Registration number:
NPCR 012:2018 Part B for Thermal insulation products
NEPD-3953-2890-EN
Issue date: 30.11.2022
Valid to: 30.11.2027
The Norwegian EPD Foundation
EPD Software:
LCA.no EPD generator
System ID:
51527
1 / 12
General information
Product Owner of the declaration:
Leca® 4-10 rund, Fibo ExClay Deutschland GmbH Leca International
Contact person: Tone Storbråten
Phone: +47 41 43 71 00
e-mail: info@leca.no
Program operator: Manufacturer:
Post Box 5250 Majorstuen, 0303 Oslo, Norway Leca International
The Norwegian EPD Foundation Årnesvegen 1 , 2009 Nordby
Phone: +47 23 08 80 00 Norway
web: post@epd-norge.no
Declaration number: Place of production:
NEPD-3953-2890-EN Leca Denmark A/S
Randersvej 75 Hinge , 8940 Randers Denmark
Denmark
Management system:
This declaration is based on Product Category Rules: ISO 14001ISO 9001
CEN Standard EN 15804:2012+A2:2019 serves as core PCR.
NPCR 012:2018 Part B for Thermal insulation products
Organisation no:
Statement of liability: 918 799 141
The owner of the declaration shall be liable for the underlying information and
evidence. EPD Norway shall not be liable with respect t​o manufacturer
information, life cycle assessment data and evidences.
Issue date: 30.11.2022
Declared unit:
1 m3 Leca® 4-10 rund, Fibo ExClay Deutschland GmbH
Valid to: 30.11.2027
Declared unit with option:
A1,A2,A3,A4,C1,C2,C3,C4,D
Year of study:
Functional unit: 2021
Comparability:
General information on verification of EPD from EPD tools: EPD of construction products may not be comparable if they not comply with
Independent verification of data, other environmental information and the EN 15804:2012+A2:2019 and seen in a building context.
declaration according to ISO 14025:2010, § 8.1.3 and § 8.1.4. Individualthird party
verification of each EPD is not required when the EPD tool is i) integrated into the
company's environmental management system, ii) the procedures for use of the
EPD tool are approved by EPDNorway, and iii)the proccess is reviewed annualy.
See Appendix G of EPD-Norway's General Programme Instructions for further
information on EPD tools.
Development and verification of EPD:
Verification of EPD tool: The declaration is created using EPD tool lca.tools ver EPD2022.03, developed by
Independent third party verification of the EPD tool, background data and test- LCA.no. The EPD tool is integrated in the company's management system, and
EPD in accordance with EPDNorway's procedures and guidelines for verification has been approved by EPD Norway.
and approval of EPD tools.
Developer of EPD:
Third party verifier:
Ana Raquel Fernandes
Reviewer of company-specific input data and EPD:​
Elisabet Amat - GREENIZE projects Tone Storbråten
(no signature required)
Approved:
2 / 12
Product
Product description:
The EPD describes results for production of lightweight expanded clay aggregate, labelled Leca®, Leca® 4-10 rund, from the factory in Hinge, Denmark. Lightweight
expanded clay aggregate is a granular ceramic material made from natural clay. The clay mixed with organic material, dried and expanded to 3-4 times its original volume
in rotary kilns at temperatures of about 1150 ° C. The output lightweight expanded clay aggregate granules, in the range 0-32 mm, are sieved and blended into different
grades of products and distributed in bulk or in bags.
The main characteristic of expanded clay is low density combined with high strength. Leca® is used for lightweight concrete, mortar, prefabricated lightweight concrete
products, lightweight fillings and other geotechnical applications. The density of Leca® 4-10 rund is 305 kg/m³. Further information or explanatory material may be
obtained by contacting Fibo ExClay Deutschland GmbH.
Product specification
Leca® 4-10 rund, natural expanded clay of various, precisely defined sizes and weights, is used as drainage and in lightweight mortars and insulating lightweight screeds.
It is also used by the processing industry as a lightweight aggregate for lightweight concrete.
Materials
Clay 92 %
Waste/bio raw materials 8 %
Lime < 0,5 %
Technical data:
Grading (Test method: EN 933-1):
4 - 10 mm
Loose bulk density (Test method: EN 1097-3):
0,305 ton/m³
Reaction to fire (2000/605/EG):
A1
Market:
Germany
Reference service life, product
Limited only by the planned service life of the final construction.
Reference service life, building or construction works
Limited only by the planned service life of the final construction.
LCA: Calculation rules
Declared unit:
1 m3 Leca® 4-10 rund, Fibo ExClay Deutschland GmbH
Cut-off criteria:
All major raw materials and all the essential energy is included. The production processes for raw materials and energy flows with very small amounts (less than 1%) are
not included. These cut-off criteria do not apply for hazardous materials and substances.
Allocation:
The allocation is made in accordance with the provisions of EN 15804+A2. Incoming energy and water and waste production in-house is allocated equally among all
products through mass allocation. Effects of primary production of recycled materials is allocated to the main product in which the material was used. The recycling
process and transportation of the material is allocated to this analysis.
Data quality:
Specific data for the product composition are provided by the manufacturer. The data represent the production of the declared product and were collected for EPD
development in the year of study. Background data is based on EPDs according to EN 15804 and different LCA databases. The data quality of the raw materials in A1 is
presented in the table below.
Materials Source Data quality Year
Additives ecoinvent 3.6 Database 2019
Binder ecoinvent 3.6 Database 2019
Dolomite ecoinvent 3.6 Database 2019
Clay LCA.no Database 2021
Waste products LCA.no Database 2021
3 / 12
System boundaries (X=included, MND=module not declared, MNR=module not relevant)
Construction Beyond the
Product stage installation Use stage End of life stage system
stage boundaries
A1 A2 A3 A4 A5 B1 B2 B3 B4 B5 B6 B7 C1 C2 C3 C4 D
X X X X MND MND MND MND MND MND MND MND X X X X X
System boundary:
Additional technical information:
waR slairetam tropsnarT gnirutcafunaM tropsnarT ylbmessA e​sU ecnanetniaM riapeR tnemecalpeR tnemhsibrufeR lanoitarepO esu ygrene lanoitarepO esu retaw -eD noitcurtsnoc noitilomed tropsnarT etsaW gnissecorp lasopsiD -yrevoceR-esueR -gnilcyceR laitnetop
4 / 12
LCA: Scenarios and additional technical information
The following information describe the scenarios in the different modules of the EPD.
Capacity utilisation Value
Transport from production place to user (A4) Distance (km) Fuel/Energy Consumption Unit
(incl. return) % (Liter/tonne)
Truck, over 32 tonnes, EURO 6 (km) 53,3 % 400 0,023 l/tkm 9,20
De-construction demolition (C1) Unit Value
Removal of LWA, Machine operation, diesel, >=
h/DU 0,04
74.57 kW (per hour)
Sorting per kg of LWA, for waste treatment after
kg/DU 305,00
removal (kg)
Capacity utilisation Value
Transport to waste processing (C2) Distance (km) Fuel/Energy Consumption Unit
(incl. return) % (Liter/tonne)
Truck, 16-32 tonnes, EURO 5 (km) 38,8 % 50 0,045 l/tkm 2,25
Waste processing (C3) Unit Value
Waste treatment, reuse of LWA (kg) kg 228,75
Disposal (C4) Unit Value
Disposal, landfilling of waste LWA (kg) kg 76,25
Benefits and loads beyond the system
Unit Value
boundaries (D)
Substitution of primary expanded clay (kg) kg 228,75
5 / 12
LCA: Results
The LCA results are presented below for the declared unit defined on page 2 of the EPD document.
Environmental impact
Parameter Unit A1 A2 A3 A4 C1 C2 C3 C4 D
GWP-total kg CO2 -eq 1,66E+00 2,42E+00 1,13E+02 1,06E+01 8,67E-01 2,54E+00 0,00E+00 6,26E-01 -5,75E+01
GWP-fossil kg CO2 -eq 1,65E+00 2,42E+00 1,12E+02 1,06E+01 8,67E-01 2,54E+00 0,00E+00 6,26E-01 -5,73E+01
GWP-biogenic kg CO2 -eq 2,00E-03 1,00E-03 6,44E-01 4,55E-03 1,61E-04 0,00E+00 0,00E+00 7,30E-04 -1,41E-01
GWP-luluc kg CO2 -eq 1,39E-04 8,60E-04 8,05E-03 3,24E-03 6,79E-05 8,89E-04 0,00E+00 1,54E-04 -2,24E-02
ODP kg CFC11 -eq 3,35E-07 5,47E-07 8,51E-07 2,56E-06 1,86E-07 5,64E-07 0,00E+00 2,37E-07 -3,37E-06
AP mol H+ -eq 3,18E-03 6,94E-03 3,43E-01 3,42E-02 3,16E-03 1,04E-02 0,00E+00 5,56E-03 -4,57E-01
EP-FreshWater kg P -eq 5,82E-06 1,93E-05 6,52E-03 8,45E-05 3,13E-06 2,00E-05 0,00E+00 7,09E-06 -2,85E-03
EP-Marine kg N -eq 5,52E-04 1,37E-03 1,32E-01 7,49E-03 1,05E-03 3,08E-03 0,00E+00 2,07E-03 -5,71E-02
EP-Terrestial mol N eq 6,38E-03 1,54E-02 1,47E+00 8,36E-02 1,16E-02 3,40E-02 0,00E+00 2,28E-02 -6,89E-01
POCP kg NMVOC -eq 2,34E-03 5,89E-03 3,47E-01 3,28E-02 3,56E-03 1,04E-02 0,00E+00 6,53E-03 -1,86E-01
ADP-minerals&metals1 Kg Sb-eq 9,90E-07 6,67E-05 2,23E-05 1,89E-04 1,32E-06 6,88E-05 0,00E+00 5,63E-06 -7,59E-04
ADP-fossil1 MJ 2,14E+01 3,65E+01 9,38E+02 1,73E+02 1,18E+01 3,83E+01 0,00E+00 1,72E+01 -5,81E+02
WDP1 m3 2,04E+02 3,53E+01 -1,90E+02 1,32E+02 2,52E+00 3,65E+01 0,00E+00 1,06E+02 -1,07E+03
GWP total Global Warming Potential total; GWP fossil Global Warming Potential fossil fuels ; GWP biogenic Global Warming Potential biogenic; GWP luluc Global W
Potential land use change; ODP Ozone Depletion; AP Acidification; EP freshwater Eutrophication aquatic freshwater; EP marine Eutrophication aquatic marine; EP
terrestrial Eutrophication terrestrial ;POCP Photochemical zone formation; ADPE Abiotic Depletion Potential minerals and metals; ADPf Abiotic Depletion Potential fossil
fuels;
"Reading example: 9,0 E-03 = 9,0*10-3 = 0,009"
*INA Indicator Not Assessed
1. The results of this environmental impact indicator shall be used with care as the uncertainties on these results are high or as there is limited experienced with the
indicator
Remarks to environmental impacts
Due to polluter-pay-principle, the emissions from waste are not included.
Biogenic carbon from biofuels are balanced to zero since they have their input and output in the same module.
6 / 12
Additional environmental impact indicators
Parameter Unit A1 A2 A3 A4 C1 C2 C3 C4 D
PM Disease incidence 9,96E-09 1,48E-07 6,39E-06 9,76E-07 6,20E-08 1,68E-07 0,00E+00 1,19E-07 -4,25E-06
IRP2 kgBq U235 eq. 1,01E-01 1,60E-01 3,44E-01 7,54E-01 5,08E-02 1,68E-01 0,00E+00 7,86E-02 -1,21E+00
ETP-fw1 CTUe 1,94E+01 2,71E+01 1,39E+03 1,26E+02 6,48E+00 2,82E+01 0,00E+00 9,39E+00 -1,40E+03
HTP-c1 CTUh 8,60E-11 0,00E+00 1,41E-08 0,00E+00 7,22E-10 0,00E+00 0,00E+00 3,81E-10 -2,56E-08
HTP-nc1 CTUh 9,76E-09 2,96E-08 1,37E-06 1,22E-07 5,15E-09 3,05E-08 0,00E+00 6,79E-09 -6,94E-07
SQP1 Pt 2,86E+00 2,56E+01 1,40E+02 1,98E+02 1,50E+00 2,64E+01 0,00E+00 6,63E+01 -8,09E+02
PM Particulate Matter emissions; IRP Ionizing radiation – human health; ETP-fw Eco toxicity – freshwater; HTP-c Human toxicity – cancer effects; HTP-nc Human
toxicity – non cancer effects; SQP Soil Quality (dimensionless)
"Reading example: 9,0 E-03 = 9,0*10-3 = 0,009"
*INA Indicator Not Assessed
1. The results of this environmental impact indicator shall be used with care as the uncertainties on these results are high or as there is limited experienced with the
indicator
2. This impact category deals mainly with the eventual impact of low dose ionizing radiation on human health of the nuclear fuel cycle. It does not consider effects due
to possible nuclear accidents, occupational exposure nor due to radioactive waste disposal in underground facilities. Potential ionizing radiation from the soil, from
radon and from some construction materials is also not measured by this indicator.
7 / 12
Resource use
Parameter Unit A1 A2 A3 A4 C1 C2 C3 C4 D
PERE MJ 6,93E-01 5,23E-01 9,53E+01 2,17E+00 6,41E-02 5,41E-01 0,00E+00 6,16E-01 -1,57E+02
PERM MJ 0,00E+00 0,00E+00 0,00E+00 0,00E+00 0,00E+00 0,00E+00 0,00E+00 0,00E+00 0,00E+00
PERT MJ 6,93E-01 5,23E-01 9,53E+01 2,17E+00 6,41E-02 5,41E-01 0,00E+00 6,16E-01 -1,57E+02
PENRE MJ 2,15E+01 3,65E+01 9,39E+02 1,73E+02 1,18E+01 3,86E+01 0,00E+00 1,72E+01 -5,81E+02
PENRM MJ 0,00E+00 0,00E+00 0,00E+00 0,00E+00 0,00E+00 0,00E+00 0,00E+00 0,00E+00 0,00E+00
PENRT MJ 2,15E+01 3,65E+01 9,39E+02 1,73E+02 1,18E+01 3,86E+01 0,00E+00 1,72E+01 -5,81E+02
SM kg 4,25E+01 0,00E+00 1,21E-01 0,00E+00 5,82E-03 1,54E-02 0,00E+00 7,47E-03 -8,59E-01
RSF MJ 1,44E-02 1,87E-02 6,76E+00 7,59E-02 1,58E-03 1,94E-02 0,00E+00 1,28E-02 -4,16E+00
NRSF MJ 6,31E-03 6,69E-02 2,24E+02 2,55E-01 2,32E-02 6,91E-02 0,00E+00 2,76E-02 -3,25E+00
FW m3 2,33E-03 3,91E-03 9,06E-02 1,96E-02 6,10E-04 4,04E-03 0,00E+00 2,12E-02 -3,86E-01
PERE Use of renewable primary energy excluding renewable primary energy resources used as raw materials; PERM Use of renewable primary energy resources used as
raw materials; PERT Total use of renewable primary energy resources; PENRE Use of non renewable primary energy excluding non-renewable primary energy resources
used as raw materials; PENRM Use of non renewable primary energy resources used as raw materials; PENRT Total use of non renewable primary energy resources; SM
Use of secondary materials; RSF Use of renewable secondary fuels; NRSF Use of non renewable secondary fuels; FW Use of net fresh water
"Reading example: 9,0 E-03 = 9,0*10-3 = 0,009"
*INA Indicator Not Assessed
8 / 12
End of life - Waste
Parameter Unit A1 A2 A3 A4 C1 C2 C3 C4 D
HWD kg 4,42E-04 1,88E-03 1,28E+00 9,44E-03 3,49E-04 1,95E-03 0,00E+00 1,21E-03 -6,40E-02
NHWD kg 1,50E-02 1,78E+00 1,62E+00 1,50E+01 1,40E-02 1,83E+00 0,00E+00 7,63E+01 -4,03E+00
RWD kg 1,55E-04 2,49E-04 2,39E-04 1,18E-03 8,22E-05 2,61E-04 0,00E+00 1,12E-04 -1,73E-03
HWD = Hazardous waste disposed; NHWD = Non-hazardous waste disposed; RWD = Radioactive waste disposed;
"Reading example: 9,0 E-03 = 9,0*10-3 = 0,009"
*INA Indicator Not Assessed
End of life - Output flow
Parameter Unit A1 A2 A3 A4 C1 C2 C3 C4 D
CRU kg 0,00E+00 0,00E+00 0,00E+00 0,00E+00 0,00E+00 0,00E+00 0,00E+00 0,00E+00 0,00E+00
MFR kg 7,59E-04 0,00E+00 1,72E-01 0,00E+00 5,71E-03 2,15E-04 2,29E+02 6,80E-03 -6,97E-01
MER kg 8,31E-04 0,00E+00 2,10E-03 0,00E+00 1,77E-05 1,28E-02 0,00E+00 1,28E-04 -4,17E-02
EEE MJ 1,37E-04 0,00E+00 3,31E+00 0,00E+00 6,07E-05 1,48E-03 0,00E+00 1,06E-02 -9,08E-02
EET MJ 2,07E-03 0,00E+00 5,01E+01 0,00E+00 9,19E-04 2,24E-02 0,00E+00 1,60E-01 -1,37E+00
CRU = Components for re-use; MFR = Materials for recycling; MER = Materials for energy recovery; EEE = Exported electrical energy; EET = Exported energy ​ Thermal
"Reading example: 9,0 E-03 = 9,0*10-3 = 0,009"
*INA Indicator Not Assessed
Biogenic Carbon Content
Parameter Unit At the factory gate
Biogenic carbon content in product kg C 0,00E+00
Biogenic carbon content in accompanying packaging kg C 0,00E+00
Note: 1 kg biogenic carbon is equivalent to 44/12 kg CO2
9 / 12
Additional Norwegian requirements
Greenhouse gas emissions from the use of electricity in the manufacturing phase
National production mix from import, low voltage (production of transmission lines, in addition to direct emissions and losses in grid) of applied electricity for the
manufacturing process (A3).
Electricity mix Data source Amount Unit
Renewable electricity Saint-Gobain, based on 100% hydro power, with Guarantee of Origin from LOS 2021 (kWh) ecoinvent 3.6 4,26 g CO2-eq/kWh
Dangerous substances
The product contains no substances given by the REACH Candidate list or the Norwegian priority list.
Indoor environment
Additional Environmental Information
Environmental impact indicators EN 15804+A1 and NPCR Part A v2.0
Parameter Unit A1 A2 A3 A4 C1 C2 C3 C4 D
GWP kg CO2 -eq 1,65E+00 2,39E+00 1,10E+02 1,05E+01 8,61E-01 2,53E+00 0,00E+00 6,13E-01 -5,60E+01
ODP kg CFC11 -eq 2,68E-07 4,44E-07 7,59E-07 2,07E-06 1,47E-07 4,58E-07 0,00E+00 1,91E-07 -2,85E-06
POCP kg C2H4-eq 2,82E-04 2,92E-04 1,35E-02 1,30E-03 1,32E-04 3,36E-04 0,00E+00 1,44E-04 -1,69E-02
AP kg SO2 -eq 2,46E-03 4,77E-03 2,41E-01 2,22E-02 1,26E-03 4,99E-03 0,00E+00 1,70E-03 -3,76E-01
EP kg PO43- -eq 2,74E-04 5,08E-04 6,30E-02 2,40E-03 1,40E-04 5,33E-04 0,00E+00 2,01E-04 -2,94E-02
ADPM kg Sb -eq 9,90E-07 6,67E-05 1,96E-05 1,89E-04 1,32E-06 6,88E-05 0,00E+00 5,63E-06 -7,59E-04
ADPE MJ 2,14E+01 3,58E+01 9,26E+02 1,69E+02 1,18E+01 3,83E+01 0,00E+00 1,65E+01 -5,54E+02
GWPIOBC kg CO2 -eq 1,65E+00 2,42E+00 1,16E+01 1,06E+01 1,98E-01 2,53E+00 0,00E+00 0,00E+00 -5,74E+01
GWP Global warming potential; ODP Depletion potential of the stratospheric ozone layer; POCP Formation potential of tropospheric photochemical oxidants; AP
Acidification potential of land and water; EP Eutrophication potential; ADPM Abiotic depletion potential for non fossil resources; ADPE Abiotic depletion​ potential for
fossil resources; GWP-IOBC/GHG Global warming potential calculated according to the principle of instantanious oxidation (except emissions and uptake of biogenic
carbon)
10 / 12
Bibliography
ISO 14025:2010 Environmental labels and declarations - Type III environmental declarations - Principles and procedures.
ISO 14044:2006 Environmental management - Life cycle assessment - Requirements and guidelines.
EN 15804:2012+A2:2019 Environmental product declaration - Core rules for the product category of construction products.
ISO 21930:2017 Sustainability in buildings and civil engineering works - Core rules for environmental product declarations of construction products.
ecoinvent v3, Allocation, cut-off by classification, Swiss Centre of Life Cycle Inventories.
Iversen et al., (2021) eEPD v2021.09 Background information for EPD generator tool system verification, LCA.no Report number: 07.21
Vold et. al., (2022) EPD generator for NPCR 012 Thermal insulation, Background information for EPD generator application and LCA data, LCA.no report number: 07.22.
NPCR Part A: Construction products and services. Ver. 2.0. April 2021, EPD-Norge.
NPCR 012 Part B for Part B for Thermal insulation products, Ver. 2.0, 31.03.2022, EPD Norway.
Program operator and publisher Phone: +47 23 08 80 00
The Norwegian EPD Foundation e-mail: post@epd-norge.no
Post Box 5250 Majorstuen, 0303 Oslo, Norway web: www.epd-norge.no
Owner of the declaration: Phone: +47 41 43 71 00
Leca International e-mail: info@leca.no
Årnesvegen 1, 2009 Nordby web: www.leca.no
Author of the Life Cycle Assessment Phone: +47 916 50 916
LCA.no AS e-mail: post@lca.no
Dokka 6B, 1671 web: www.lca.no
Developer of EPD generator Phone: +47 916 50 916
LCA.no AS e-mail: post@lca.no
Dokka 6B,1671 Kråkerøy web: www.lca.no
ECO Platform Web: www.eco-platform.org
ECO Portal Web: ECO Portal
11 / 12
EPD for the best
environmental
decision
The Norwegian EPD Foundation
www.epd-norge.no
12 / 12
