Environmental product declaration
in accordance with ISO 14025 and EN 15804+A2
JACKOFOAM GRUNNMURSPLATE XPS NORWAY
Owner of the declaration: Program operator:
Bewi Insulation Scandinavia The Norwegian EPD Foundation
Product: Declaration number:
JACKOFOAM GRUNNMURSPLATE XPS NORWAY
Registration number:
Declared unit:
1 m2 Issue date:
This declaration is based on Product Category Rules: Valid to:
CEN Standard EN 15804:2012+A2:2019 serves as core
EPD Software:
PCR
The Norwegian EPD Foundation LCA.no EPD generator ID: 74530
NPCR 012:2022 Part B for Thermal insulation products
1 / 12
General information
Product Owner of the declaration:
JACKOFOAM GRUNNMURSPLATE XPS NORWAY Bewi Insulation Scandinavia
Contact person: Svein Tore Larsen
Phone: +47 95 07 67 42
e-mail: svein.tore.larsen@jackon.no
Program operator: Manufacturer:
Post Box 5250 Majorstuen, 0303 Oslo, Norway Bewi Insulation Scandinavia
The Norwegian EPD Foundation Sørkilen 3
Phone: +47 23 08 80 00 1621 GRESSVIK, Fredrikstad i VIKEN, Norway
web: post@epd-norge.no
Declaration number: Place of production:
Bewi Insulation Scandinavia, Fredrikstad
Sørkilen 3
NO-1621 Gressvik, Norway
This declaration is based on Product Category Rules: Management system:
CEN Standard EN 15804:2012+A2:2019 serves as core PCR ISO 9001: 185977-2015-AQ-NOR-NA and ISO 14001: 251411-
NPCR 012:2022 Part B for Thermal insulation products 2017-AE-NOR-NA
Statement of liability: Organisation no:
The owner of the declaration shall be liable for the underlying 913019334
information and evidence. EPD Norway shall not be liable with respect
to manufacturer information, life cycle assessment data and
evidences.​
Declared unit: Issue date:
1 m2 JACKOFOAM GRUNNMURSPLATE XPS NORWAY
Declared unit with option: Valid to:
A1,A2,A3,A4,A5,C1,C2,C3,C4,D
Year of study:
2021
Declared unit, specification: Comparability:
1 m² Jackofoam 300 XPS cellar wall insulation board with 34 mm EPD of construction products may not be comparable if they not
thickness at R=1 m² comply with EN 15804 and seen in a building context.
K/W, transportation to site, waste handling and recovery.
General information on verification of EPD from EPD tools: Development and verification of EPD:
Independent verification of data, other environmental information The declaration is created using EPD tool lca.tools ver EPD2022.03,
and the declaration according to ISO 14025:2010, § 8.1.3 and § 8.1.4. developed by LCA.no. The EPD tool is integrated in the company's
Verification of each EPD is made according to EPD-Norway’s management system, and has been approved by EPD Norway.
guidelines for verification and approval requiring that tools are i)
integrated into the company's environmental management system, ii) Developer of EPD: Jostein Häckert
the procedures for use of the EPD tool are approved by EPD-Norway,
Reviewer of company-specific input data and EPD:​ Svein Tore Larsen
and iii) the process is reviewed annually by an independent third
party verifier. See Appendix G of EPD-Norway's General Programme
Instructions for further information on EPD tools
Verification of EPD tool: Approved:
Independent third party verification of the EPD tool, background data
and test-EPD in accordance with EPDNorway's procedures and
guidelines for verification and approval of EPD tools.
Third party verifier:
Elisabet Amat, GREENIZE projects
(no signature required)
2 / 12
Product
Product description:
The insulation board is provided in several dimensions and thicknesses. Please use the conversion table below for other sizes than the declared
unit.
Extruded polystyrene (XPS) is a common material used for thermal insulation of buildings and constructions. It's a polymer foam, consisting of
airfilled polystyrene cells. As most of the material is air, XPS provides good insulating properties at a low weight. Other characteristics of the
material
include low moisture absorption, long service life and high compressive strength.
This LCA is based on Jackofoam 300 and can be used for all Jackofoam products with the conversion factor which can be found under System
boundaries.
Product specification
XPS is manufactured through an extruder where polystyrene granulates are mixed with additives and foaming
agents to produce the foam mass. The foam mass is pressed out flat to a board through a nozzle in deisre thickness and cut into correct
dimensions. Some of the remaining blowing agents are aired out before the product leaves the factory gate.
The number of the product is the pressure class; here 300 which means a short dermation of 10% when the load of the product is 300 kN/m2.
Weight per declared unit is 1,3807 kg given a density of 31,5 kg/cubic meter with a thickness of 34 mm including non woven fabric geotextil and
packaging material.
Materials kg %
Adhesive 0,00 0,07
Expansion gas 0,09 6,76
Others 0,17 12,76
Plastic - Polystyrene expandable (EPS) 1,07 80,40
Total 1,33
Packaging kg %
Packaging - Plastic 0,03 14,70
Packaging - Wood 0,15 85,30
Total incl. packaging 1,51
Technical data:
CE marking: XPS insulation boards are CE certified according to NS-EN 13164
Typical size: 585 mm x 1185 mm, 585 x 2385 mm
Typical thickness: 50 mm - 150 mm
Moisture absorption: <0,7 vol%
Density:
Jackofoam 250: 30,0 kg/m3
Jackofoam 300: 31,5 kg/m3
Jackofoam 400: 34,0 kg/m3
Jackofoam 500: 37,5 kg/m3
Jackofoam 700: 48,0 kg/m3
Market:
Norway, Sweden
Reference service life, product
As in the construction where it is used.
Reference service life, building or construction works
As in the construction where it is used.
LCA: Calculation rules
Declared unit:
1 m2 JACKOFOAM GRUNNMURSPLATE XPS NORWAY
Cut-off criteria:
All major raw materials and all the essential energy is included. The production processes for raw materials and energy flows with very small
amounts (less than 1%) are not included. These cut-off criteria do not​ apply for hazardous materials and substances.
Allocation:
3 / 12
The allocation is made in accordance with the provisions of EN 15804. Incoming energy and water and waste production in-house is allocated
equally among all products through mass allocation. Effects of primary production of recycled materials is allocated to the main product in which
the material was used. The recycling process and transportation of the material is allocated to this analysis.
Data quality:
Specific data for the product composition are provided by the manufacturer. The data represent the production of the declared product and were
collected for EPD development in the year of study. Background data is based on EPDs according to EN 15804 and different LCA databases. The
data quality of the raw materials in A1 is presented in the table below.
Materials Source Data quality Year
Adhesive ecoinvent 3.6 Database 2019
Expansion gas ecoinvent 3.6 Database 2019
Others ecoinvent 3.6 Database 2019
Packaging - Plastic ecoinvent 3.6 Database 2019
Packaging - Wood ecoinvent 3.6 Database 2019
Expansion gas ecoinvent 3.6 Database 2020
European
Plastic - Polystyrene expandable (EPS) Plastics Europe + ecoinvent 3.6 2019
average.
4 / 12
System boundaries (X=included, MND=module not declared, MNR=module not relevant)
Construction Beyond the system
Product stage Use stage End of life stage
installation stage boundaries
A1 A2 A3 A4 A5 B1 B2 B3 B4 B5 B6 B7 C1 C2 C3 C4 D
X X X X X MNR MNR MNR MNR MNR MNR MNR X X X X X
System boundary:
Additional technical information:
waR slairetam tropsnarT gnirutcafunaM tropsnarT ylbmessA e​sU ecnanetniaM riapeR tnemecalpeR tnemhsibrufeR lanoitarepO ygrene esu lanoitarepO esu retaw -eD noitcurtsnoc noitilomed tropsnarT etsaW gnissecorp lasopsiD -yrevoceR-esueR laitnetop-gnilcyceR
5 / 12
LCA: Scenarios and additional technical information
The following information describe the scenarios in the different modules of the EPD.
Capacity utilisation Value
Transport from production place to user (A4) Distance (km) Fuel/Energy Consumption Unit
(incl. return) % (Liter/tonne)
Truck, 16-32 tonnes, EURO 6 (kgkm) 36,7 % 300 0,043 l/tkm 12,90
Assembly (A5) Unit Value
Waste, packaging, plastic to average treatment -
kg 0,03
A5 (inkl transport) (kg)
Waste, packaging, wood to average treatment -
kg 0,15
A5 (inkl transport) (kg)
De-construction demolition (C1) Unit Value
Manual demolition of EPS in C1 kg/DU 1,33
Capacity utilisation Value
Transport to waste processing (C2) Distance (km) Fuel/Energy Consumption Unit
(incl. return) % (Liter/tonne)
Truck, over 32 tonnes, EURO 6 (kgkm) - RER 53,3 % 83 0,023 l/tkm 1,91
Waste processing (C3) Unit Value
Waste, Polystyrene, incineration kg 1,33
Disposal (C4) Unit Value
Landfilling of ashes from incineration of PS kg 0,00
Benefits and loads beyond the system
Unit Value
boundaries (D)
substitution of electricity, Norway MJ 0,88
Substitution of thermal energy, Norway (MJ) MJ 44,13
6 / 12
LCA: Results
The LCA results are presented below for the declared unit defined on page 2 of the EPD document.
Environmental impact
Indicator Unit A1 A2 A3 A4 A5 C1 C2 C3 C4 D
GWP-total
kg CO2 -
2,88E+00 1,70E-01 5,77E-02 6,53E-02 6,28E-03 0,00E+00 9,63E-03 4,24E+00 2,07E-04 -2,51E-01
eq
GWP-fossil
kg CO2 -
3,10E+00 1,70E-01 5,33E-02 6,52E-02 6,26E-03 0,00E+00 9,62E-03 4,24E+00 2,07E-04 -2,43E-01
eq
GWP-biogenic
kg CO2 -
-2,22E-01 7,18E-05 4,27E-03 2,70E-05 2,05E-05 0,00E+00 4,12E-06 2,93E-05 1,10E-07 -1,59E-04
eq
GWP-luluc
kg CO2 -
1,29E-03 5,32E-05 9,71E-05 2,32E-05 1,23E-06 0,00E+00 2,93E-06 4,64E-06 3,17E-08 -8,76E-03
eq
kg
ODP CFC11 - 6,06E-08 4,06E-08 1,91E-09 1,48E-08 7,90E-10 0,00E+00 2,32E-09 3,04E-09 2,20E-11 -1,86E-02
eq
mol H+
AP 7,24E-03 6,44E-04 1,10E-04 1,87E-04 3,60E-05 0,00E+00 3,10E-05 5,05E-04 7,28E-07 -2,00E-03
-eq
EP-FreshWater kg P -eq 3,01E-05 1,34E-06 1,08E-06 5,21E-07 5,41E-08 0,00E+00 7,66E-08 3,00E-07 2,79E-09 -2,18E-05
EP-Marine kg N -eq 1,71E-03 1,42E-04 2,77E-05 3,71E-05 1,67E-05 0,00E+00 6,79E-06 2,43E-04 2,27E-07 -6,78E-04
mol N -
EP-Terrestial 1,87E-02 1,59E-03 2,64E-04 4,15E-04 1,63E-04 0,00E+00 7,57E-05 2,60E-03 2,59E-06 -7,30E-03
eq
kg
POCP NMVOC 7,82E-03 5,82E-04 4,39E-03 1,59E-04 4,25E-05 0,00E+00 2,97E-05 6,23E-04 7,14E-07 -2,02E-03
-eq
ADP- kg Sb -
9,21E-06 3,15E-06 6,13E-07 1,80E-06 7,85E-08 0,00E+00 1,71E-07 1,31E-07 1,16E-09 -1,55E-06
minerals&metals1 eq
ADP-fossil1 MJ 1,03E+02 2,73E+00 3,49E-01 9,86E-01 5,75E-02 0,00E+00 1,56E-01 2,60E-01 1,88E-03 -3,48E+00
WDP1 m3 1,85E+01 2,12E+00 5,56E+01 9,54E-01 1,06E-01 0,00E+00 1,20E-01 5,77E-01 1,95E-02 -1,38E+01
GWP-total = Global Warming Potential total; GWP-fossil = Global Warming Potential fossil fuels; GWP-biogenic = Global Warming Potential biogenic; GWP-luluc =
Global Warming Potential land use and land use change; ODP = Depletion potential of the stratospheric ozone layer; AP = Acidification potential, Accumulated
Exceedance; EP-freshwater = Eutrophication potential, fraction of nutrients reaching freshwater end compartment: EP-marine = Eutrophication potential, fraction of
nutrients reaching marine end compartment; EP-terrestrial = Eutrophication potential, Accumulated Exceedance; POCP = Formation potential of tropospheric ozone;
ADP-minerals&metals = Abiotic depletion potential for non-fossil resources; ADP-fossil = Abiotic depletion for fossil resources potential; WDP = Water (user)
deprivation potential, deprivation-weighted water consumption
"Reading example: 9,0 E-03 = 9,0*10-3 = 0,009"
*INA Indicator Not Assessed
1. The results of this environmental impact indicator shall be used with care as the uncertainties on these results are high or as there is limited experienced with the
indicator
Remarks to environmental impacts
7 / 12
Additional environmental impact indicators
Indicator Unit A1 A2 A3 A4 A5 C1 C2 C3 C4 D
PM Disease incidence 5,80E-08 1,49E-08 1,03E-09 3,99E-09 4,55E-10 0,00E+00 8,84E-10 2,13E-09 9,00E-12 -1,27E-07
IRP2 kgBq U235 -eq 8,21E-02 1,19E-02 5,96E-03 4,31E-03 2,16E-04 0,00E+00 6,83E-04 4,35E-04 8,93E-06 -2,01E-02
ETP-fw1 CTUe 4,11E+02 1,99E+00 6,47E-01 7,31E-01 6,38E-02 0,00E+00 1,14E-01 6,27E-01 3,46E-03 -1,91E+01
HTP-c1 CTUh 1,26E-09 0,00E+00 3,70E-11 0,00E+00 6,00E-12 0,00E+00 0,00E+00 1,78E-10 0,00E+00 -3,26E-10
HTP-nc1 CTUh 4,87E-08 1,94E-09 8,24E-10 7,99E-10 3,05E-10 0,00E+00 1,10E-10 7,05E-09 6,00E-12 -1,81E-08
SQP1 dimensionless 2,85E+01 2,97E+00 1,66E-01 6,90E-01 4,25E-02 0,00E+00 1,79E-01 3,10E-02 5,19E-03 -2,44E+01
PM = Particulate Matter emissions; IRP = Ionizing radiation – human health; ETP-fw = Eco toxicity – freshwater; HTP-c = Human toxicity – cancer effects; HTP-nc =
Human toxicity – non cancer effects; SQP = Potential Soil Quality Index (dimensionless)
"Reading example: 9,0 E-03 = 9,0*10-3 = 0,009"
*INA Indicator Not Assessed
1. The results of this environmental impact indicator shall be used with care as the uncertainties on these results are high or as there is limited experienced with the
indicator
2. This impact category deals mainly with the eventual impact of low dose ionizing radiation on human health of the nuclear fuel cycle. It does not consider effects due
to possible nuclear accidents, occupational exposure nor due to radioactive waste disposal in underground facilities. Potential ionizing radiation from the soil, from
radon and from some construction materials is also not measured by this indicator.
8 / 12
Resource use
Indicator Unit A1 A2 A3 A4 A5 C1 C2 C3 C4 D
PERE MJ 2,48E+00 3,45E-02 4,09E+00 1,41E-02 1,22E-03 0,00E+00 1,97E-03 7,48E-03 1,10E-04 -2,02E+01
PERM MJ 2,14E+00 0,00E+00 0,00E+00 0,00E+00 0,00E+00 0,00E+00 0,00E+00 0,00E+00 0,00E+00 0,00E+00
PERT MJ 4,62E+00 3,45E-02 4,09E+00 1,41E-02 1,22E-03 0,00E+00 1,97E-03 7,48E-03 1,10E-04 -2,02E+01
PENRE MJ 7,27E+01 2,73E+00 3,50E-01 9,86E-01 5,75E-02 0,00E+00 1,56E-01 2,60E-01 1,88E-03 -3,48E+00
PENRM MJ 3,57E+01 0,00E+00 0,00E+00 0,00E+00 0,00E+00 0,00E+00 0,00E+00 0,00E+00 0,00E+00 0,00E+00
PENRT MJ 1,08E+02 2,73E+00 3,50E-01 9,86E-01 5,75E-02 0,00E+00 1,56E-01 2,60E-01 1,88E-03 -3,48E+00
SM kg 2,21E-03 0,00E+00 0,00E+00 0,00E+00 4,15E-06 0,00E+00 0,00E+00 0,00E+00 0,00E+00 0,00E+00
RSF MJ 2,21E-02 1,21E-03 3,51E-03 5,05E-04 3,50E-05 0,00E+00 6,88E-05 2,09E-04 2,73E-06 -2,10E-03
NRSF MJ 1,67E-03 4,06E-03 8,79E-03 1,81E-03 3,48E-04 0,00E+00 2,31E-04 0,00E+00 4,34E-04 -1,34E+00
FW m3 7,65E-02 3,05E-04 3,52E-02 1,05E-04 4,01E-05 0,00E+00 1,78E-05 7,36E-04 1,73E-06 -9,59E-03
PERE = Use of renewable primary energy excluding renewable primary energy resources used as raw materials; PERM = Use of renewable primary energy resources used
as raw materials; PERT = Total use of renewable primary energy resources; PENRE = Use of non renewable primary energy excluding non-renewable primary energy
resources used as raw materials; PENRM = Use of non renewable primary energy resources used as raw materials; PENRT = Total use of non renewable primary energy
resources; SM = Use of secondary materials; RSF = Use of renewable secondary fuels; NRSF = Use of non-renewable secondary fuels; FW = Net use of fresh water
"Reading example: 9,0 E-03 = 9,0*10-3 = 0,009"
*INA Indicator Not Assessed
9 / 12
End of life - Waste
Indicator Unit A1 A2 A3 A4 A5 C1 C2 C3 C4 D
HWD kg 4,71E-03 1,48E-04 6,44E-03 5,09E-05 3,43E-06 0,00E+00 8,55E-06 0,00E+00 3,43E-03 -5,50E-05
NHWD kg 1,07E-01 2,23E-01 3,38E-02 4,80E-02 1,68E-01 0,00E+00 1,36E-02 0,00E+00 1,70E-03 -7,24E-02
RWD kg 3,28E-05 1,87E-05 3,07E-06 6,72E-06 5,84E-08 0,00E+00 1,07E-06 0,00E+00 1,13E-08 -1,75E-05
HWD = Hazardous waste disposed; NHWD = Non-hazardous waste disposed; RWD = Radioactive waste disposed
"Reading example: 9,0 E-03 = 9,0*10-3 = 0,009"
*INA Indicator Not Assessed
End of life - Output flow
Indicator Unit A1 A2 A3 A4 A5 C1 C2 C3 C4 D
CRU kg 0,00E+00 0,00E+00 0,00E+00 0,00E+00 0,00E+00 0,00E+00 0,00E+00 0,00E+00 0,00E+00 0,00E+00
MFR kg 1,06E-03 0,00E+00 2,30E-02 0,00E+00 1,36E-02 0,00E+00 0,00E+00 0,00E+00 0,00E+00 0,00E+00
MER kg 2,41E-04 0,00E+00 2,21E-07 0,00E+00 1,54E-01 0,00E+00 0,00E+00 1,33E+00 0,00E+00 0,00E+00
EEE MJ 1,25E-03 0,00E+00 2,23E-02 0,00E+00 1,07E-01 0,00E+00 0,00E+00 2,35E+00 0,00E+00 0,00E+00
EET MJ 1,89E-02 0,00E+00 3,37E-01 0,00E+00 1,63E+00 0,00E+00 0,00E+00 3,55E+01 0,00E+00 0,00E+00
CRU = Components for re-use; MFR = Materials for recycling; MER = Materials for energy recovery; EEE = Exported energy electrical; EET = Exported energy thermal
"Reading example: 9,0 E-03 = 9,0*10-3 = 0,009"
*INA Indicator Not Assessed
Biogenic Carbon Content
Indicator Unit At the factory gate
Biogenic carbon content in product kg C 0,00E+00
Biogenic carbon content in accompanying packaging kg C 6,38E-02
Note: 1 kg biogenic carbon is equivalent to 44/12 kg CO2
10 / 12
Additional requirements
Greenhouse gas emissions from the use of electricity in the manufacturing phase
National production mix from import, low voltage (production of transmission lines, in addition to direct emissions and losses in grid) of applied
electricity for the manufacturing process (A3).
Electricity mix Data source Amount Unit
Electricity, Norway (kWh) ecoinvent 3.6 21,18 g CO2-eq/kWh
Dangerous substances
The product contains no substances given by the REACH Candidate list.
Indoor environment
Additional Environmental Information
Additional environmental impact indicators required in NPCR Part A for construction products
Indicator Unit A1 A2 A3 A4 A5 C1 C2 C3 C4 D
GWPIOBC kg CO2 -eq 6,31E-01 1,70E-01 3,84E-02 6,53E-02 0,00E+00 0,00E+00 9,63E-03 4,24E+00 2,15E-04 -2,48E-01
GWP-IOBC: Global warming potential calculated according to the principle of instantaneous oxidation. In order to increase the transparency of biogenic carbon​
contribution to climate impact, the indicator GWP-IOBC is required as it declares climate impacts calculated according to the principle of instantaneous oxidation.​
GWP-IOBC is also referred to as GWP-GHG in context to Swedish public procurement legislation.
11 / 12
Bibliography
ISO 14025:2010 Environmental labels and declarations - Type III environmental declarations - Principles and procedures.
ISO 14044:2006 Environmental management - Life cycle assessment - Requirements and guidelines.
EN 15804:2012+A2:2019 Environmental product declaration - Core rules for the product category of construction products.
ISO 21930:2017 Sustainability in buildings and civil engineering works - Core rules for environmental product declarations of construction
products.
ecoinvent v3, Allocation, cut-off by classification, Swiss Centre of Life Cycle Inventories.
Iversen et al., (2021) eEPD v2021.09 Background information for EPD generator tool system verification, LCA.no Report number: 07.21
Vold, M. et al (2022): EPD generator for NPCR 012, Additional products, EPS and XPS, Background information for EPD generator application
NPCR Part A: Construction products and services. Ver. 2.0. April 2021, EPD-Norge.
NPCR 012 Part B for Thermal insulation products, version 2, 31.03.2022, 2022., EPD Norway.
Program operator and publisher Phone: +47 23 08 80 00
The Norwegian EPD Foundation e-mail: post@epd-norge.no
Post Box 5250 Majorstuen, 0303 Oslo, Norway web: www.epd-norge.no
Owner of the declaration: Phone: +47 95 07 67 42
Bewi Insulation Scandinavia e-mail: svein.tore.larsen@jackon.no
Sørkilen 3, 1621 GRESSVIK, Fredrikstad i VIKEN web: www.jackon.no
Author of the Life Cycle Assessment Phone: +47 916 50 916
LCA.no AS e-mail: post@lca.no
Dokka 6B, 1671 web: www.lca.no
Developer of EPD generator Phone: +47 916 50 916
LCA.no AS e-mail: post@lca.no
Dokka 6B,1671 Kråkerøy web: www.lca.no
ECO Platform web: www.eco-platform.org
ECO Portal web: ECO Portal
12 / 12
