Environmental Product
Declaration
In accordance with ISO 14025 and EN 15804 +A2
Owner of the declaration: Product name
Lyngson SIA
LISA 22-070-2500
Program holder and
publisher: The Norwegian EPD
foundation
Manufacturer
Declaration number:
NEPD-4527-3783
-EN
Registration Number:
NEPD-4527-3783
-EN
Issue date:
Valid to:
The Norwegian 04.08.2023
EPD Foundation 04.08.2028
ver-120224
General information
Product:
LISA 22-070-2500 Owner of the declaration:
Lyngson SIA
Program Operator: Contact person:
The Norwegian EPD Foundation
Uldis Benhens
Post Box 5250 Majorstuen, 0303 Oslo, Norway
+371 29 47 47 39
Tlf: +47 23 08 80 00
Uldis.Benhens@lyngson.lv
e-mail: post@epd-norge.no
Manufacturer:
Declaration Number:
Lyngson SIA
NEPD-4527-3783
"Akači", Grēnes, Olaines novads, Latvija
+371 67 79 67 10
-EN
This declaration is based on Product
info@lyngson.lv
Category Rules:
EN 15804:2012+A2:2019 Place of production:
"Akači", Grēnes, Olaines novads, Latvija
and NPCR Part A
Construction products and services ver 2.
Statements: Management system:
The owner of the declaration shall be liable for the ISO 9001, ISO 14001, ISO 50001
underlying information and evidence. EPD
Norway shall not be liable with respect to Organisation no:
manufacturer, life cycle assessment data and LV40003822806
evidences.
Issue date:
Declared unit:
1 piece of LISA Panel radiator type 22 size
– H70mm x L2500mm, capable to produce 1 kW 04.08.2023
Valid to:
of heating as defined by the manufacturer
Verification: 04.08.2028
Year of study:
Independent verification of the declaration
2023
and data, according to ISO14025:2010
Comparability:
internal external ⊠ EPDs from other programmes than EPD Norge may
Signature
not be comparable.
The EPD has been worked out by:
Bureau Veritas Latvia
Elisabet Amat
Independent verifier approved by EPD Norway
Approved (Manager of EPD Norway)
EPD for the best environmental decision 2
Product
Product description:
Radiator/convector LISA 22-070-2500 is produced out of steel plates and rectangular steel pipes
as a panel heater with external connection of thermostat and side connections to the
infrastructure of the heating systems. These devices have a wide range of applications in closed
environments, both in new construction and renovations.
Product specification:
The product composition is Steel and Coating powder.
Products materials KG %
Steel 17,24 97,0
Coating powder 0,54 3,0
TOTAL 17,78 100,0
Packaging materials KG %
Polyethylene film 0,36 17,6
Cardboard 0,49 23,9
Wooden pallets 1,20 58,5
TOTAL 2,05 100,0
Technical data:
• Length – 2500 mm, Height – 70 mm, Width – 92 mm
• Thickness of steel pipes – 1.8 mm
• Weight of the product (w/o packaging) - 17,78 kg
• Reference lifetime - 50 years (per PSR-0011)
• Max working pressure – 6 bar (for greater pressure values consult with manufacturer)
Market:
Sweden, Norway, Denmark, and Finland
Reference service life, product:
50 years according to PSR-0011-ed1.0-EN-2018 02 09
EPD for the best environmental decision 3
LCA: Calculation rules
Functional/Declared unit:
Functional unit is taken as PSR-0011-ed1.0-EN-2018 02 09 foresees: “To produce 1 kW of heating
as defined by the manufacturer, according to the reference usage scenario and during the 50-year
reference lifetime of the product”. Therefore the Functional unit is “1 piece of LISA Panel radiator
type 22 size – h70 mm x L2500mm, capable to produce 1 kW of heating as defined by the
manufacturer” according to EN 442.
Data quality:
The production data are from 2022, the database data are from 2013 – 2021 i.e. no data is older
than 10 years. Database used is mainly Ecoinvent v3.8, with an addition of Carbon Minds 2022.01.
The LCA software used is SimaPro 9.4.
Allocation:
General allocation principles were applied according to ISO 14044:2006 4.3.4 and in line with the
provisions of EN 15804:2012+A2. Incoming energy, water and generation of waste are allocated
equally among all products through mass allocation. The material and energy consumption in
manufacturers’ data according to recorded production is also indicated per piece of the products
produced as radiator that is able to produce 1 kW of heat is of specific dimensions and weight of
materials. The effects of primary production of recycled materials has been allocated to the main
product in which the material has been used. LISA Hot Water radiators are produced only in one
manufacturing plant.
System boundary:
LCA has been performed as “Cradle-to-gate with options, modules C1-C4 and module D”,
including also module A4. All major materials, resource and energy use in manufacturing, as well
as waste are included for phases A1-A3, A4, C1-C4 and D, see flowchart below. The following
information describes the scenarios in the different modules of the EPD.
EPD for the best environmental decision 4
Cut-off criteria:
All materials have been accounted for in the LCA according to the data provided by manufacturer.
There is no missing data for processes in the system boundaries. All the materials and processes,
which have been accounted for by the manufacturing company for the relevant manufacturing
process are included in the LCI. Flows excluded from the study because of the insignificance and
difficulty of attributing them to a particular reference product are listed below:
• Copper scrap from sharpening of electrodes (0.001 kg)
General cut-off criteria are given in standard EN 15804:2012+A2, clause 6.3.6. This cut-off rule
does not apply for hazardous materials and substances and it is consistent with EN 15804+A2.
Infrastructure processes, e.g. manufacturing and maintenance of facilities and manufacturing
equipment, have been excluded from this LCA study.
EPD for the best environmental decision 5
LCA: Scenarios and additional technical information
The following information describe the scenarios in the different modules of the EPD.
Product stage (A1, A2, A3)
- Raw material supply (A1)
In module A1 extraction and processing of raw materials and generation of electricity and heat
from primary energy resources for the production of these raw materials are included. Main raw
material for production of HW radiator/convector LISA is steel pipes and plates. For
manufacturing of the product, Coating powder also is required.
- Transport of raw materials (A2)
For module A2, the transportation of raw materials and packaging materials to the production
plant, the following assumptions have been made (see Table below). According to manufacturer
provided data, EURO6 emission standard has been applied as a standard value for all Freight
lorries, with only exception of local supplier of wooden pallets and Freight lorry of lower capacity
(7.5-16 t). For some materials additional transportation mode of Light commercial vehicle has
been used.
Steel is transported from 3 different suppliers that are located in European Union (EU). Packaging
materials and other ancillary materials are supplied both locally and from countries of EU.
Material Type of vehicle Weight, kg per FU Distance, km kg*km
Steel pipes Lorry 16-32t, EURO6 1,19E+01 1880 2,24E+04
Steel coil Lorry 16-32t, EURO6 3,95E+00 545 2,15E+03
Steel PLATE Lorry 16-32t, EURO6 2,57E+00 30 7,72E+01
Oil for maintanance Light commercial vehicle 6,86E-03 30 2,06E-01
Cooling liquid Light commercial vehicle 2,15E-03 30 6,45E-02
Chemicals for washing Light commercial vehicle 6,95E-04 30 2,09E-02
Coating powder Lorry 16-32t, EURO6 5,40E-01 25 1,35E+01
Plastic plugs Light commercial vehicle 2,00E-02 36 7,02E-01
PE packaging film Light commercial vehicle 3,60E-01 3 1,08E+00
Gardobond additives Lorry 16-32t, EURO6 3,87E-02 550 2,13E+01
EU pallets Lorry 7.5-16t, EURO5 1,20E+00 3 3,60E+00
Cardbord Lorry 16-32t, EURO6 4,90E-01 300 1,47E+02
- Manufacturing (A3)
The manufacturing of the product (module A3) includes several stages of metal processing such
as stamping, welding, degreasing, powder coating, drying and then the assembling and packing
of the final product. LISA HW radiators are produced within the limits of the same plant. Local
mix of Electricity is one of the main source of energy for manufacturing purposes. Natural gas is
used for the purpose of Heat production in powder coating process. Internal transportation of
materials and product is organized with Electric skid-steer loaders, therefore, no Diesel
consumption has been declared by manufacturer.
EPD for the best environmental decision 6
In 2021 Lygson SIA installed one of the largest solar panel parks in Latvia. Within the project,
1700+ solar panels with the total capacity of 560 kW were installed on the roof of the
manufacturing plant. According to manufacturer provided data, solar panels cover 23% share of
the company’s own consumption of electricity. Electricity generated from solar panel park is used
for the production needs.
Not all materials are used to full potential, therefore, some waste flows are produced during the
manufacturing phase. Types of waste, created in the manufacturing process, are related to the
packaging of the incoming raw materials and main raw material – Steel (production waste).
Waste packaging materials, i.e. all sorts of Plastics, Wood, Cardboard and Steel, that are coming
with Raw materials declared in module A1, are collected at the gate of the manufacturer by the
waste treatment company. The wastewater is treated by local wastewater treatment company,
that has specific requirements for contents of wastewater coming from manufacturer.
The secondary material used in the final product is Steel – according to manufacturer provided
data, recycled share of incoming Steel ranges from 20% to 80% depending on supplier and type
of material, i.e. Steel plate and Steel pipe. For the purpose of this study Steel plates are
represented by Unalloyed steel (converter production), that has 23% of post-consumer material
(iron scrap), while Steel coil and Steel pipes are represented by Low-alloyed steel (electric
production), that has 85% of post-consumer material (iron scrap).
Manufacturing process for LISA HW radiator foresees the use of Coating powder and ancillary
materials, i.e. cleaning agents, maintenance oil and degreasers. Safety Data Sheets (SDS) have
been provided on all chemicals used in module A3.
Transport from production place to assembly/user (A4)
Module A4 contains the scenarios defined by manufacturer and includes transportation from
production site in Latvia, Olaine to customers, including 200km radius:
- 46.5% trade towards Stockholm, Sweden with 354 km distance for Road transport and
281 km for Sea transport
- 32.5% trade towards Oslo, Norway with 840 km distance for Road transport and 281 km
for Sea transport
- 2.4% trade towards Helsinki, Finland with 437 km distance for Road transport and 85 km
for Sea transport;
- 18.6% trade towards Copenhagen, Denmark with 578 km distance for Road transport and
404 km for Sea transport;
Following table represents capacity utilisation rates that have been used in the model due to
limitations of Ecoinvent database. Real capacity utilisation rates, provided by manufacturer, are
as follows:
- 90% capacity utilisation rate for Stockholm, Sweden
- 95% capacity utilisation rate for Oslo, Norway
- 90% capacity utilisation rate for Helsinki, Finland
- 90% capacity utilisation rate for Copenhagen, Denmark
EPD for the best environmental decision 7
Capacity utilisation (incl. Distance Fuel/Energy value
Type Type of vehicle
return) % KM consumption (l/t)
Stockholm, Sweden
Default value from
Road Lorry, >32t, EURO6 354 0,0226 l/tkm 7,99
Ecoinvent 3.8
Default value from
Water Sea ferry 281 0,0298 l/tkm 8,37
Ecoinvent 3.8
Oslo, Norway
Default value from
Road Lorry, >32t, EURO6 840 0,0226 l/tkm 18,97
Ecoinvent 3.8
Default value from
Water Sea ferry 281 0,0298 l/tkm 8,37
Ecoinvent 3.8
Helsinki, Finland
Default value from
Road Lorry, >32t, EURO6 437 0,0226 l/tkm 9,87
Ecoinvent 3.8
Default value from
Water Sea ferry 85 0,0298 l/tkm 2,53
Ecoinvent 3.8
Copenhagen, Denmark
Default value from
Road Lorry, >32t, EURO6 578 0,0226 l/tkm 13,05
Ecoinvent 3.8
Default value from
Water Sea ferry 404 0,0298 l/tkm 12,03
Ecoinvent 3.8
Assembly (A5)
Module A5 has not been declared in this study.
End of Life (C1, C3, C4)
- Demolition (C1)
It has been assumed that no particular activities in module C1 are causing a relevant
environmental impact within the demolition or the disassembling of a LISA HW radiator before
its transportation to waste processing.
- Waste processing (C3)
As a waste processing activity in module C3, recycling, i.e. sorting of Scrap steel, has been
considered, as per PSR-0011. Recycling represents 99% share of the product weight with
remaining 1% representing Scrap steel and Paint for Incineration treatment in module C4 only
as a method of final disposal.
- Disposal (C4)
Module C4 represents Incineration activities for final disposal of 1% share of the product. As
Ecoinvent v3.8 scrap steel incineration dataset suggests, 472.89 grams of 1kg of incineration
residue represents recyclable amount of Steel scrap that has been also considered in module D
as an addition to Recycled amount of the product. Incineration is carried out without energy
recovery and is considered only as a method of waste disposal.
EPD for the best environmental decision 8
Type Unit Value
Hazardous waste disposed kg 0
Collected as mixed construction waste kg 0
Reuse kg 0
Recycling kg 17,69
Energy recovery kg 0,0
To landfill kg 0,09
Transport to waste processing (C2)
For module C2 an average transportation with 100km distance has been assumed, as suggested
by PSR-0011-ed1.0-EN-2018 02 09. EURO6 16-32t Freight lorry has been used for calculations in
module C2.
Benefits and loads beyond the system boundaries (D)
As described above, this study also considers module D, where benefits and loads associated with
avoided product, i.e. Steel, have been considered, also taking into account post-consumer
material share in the product.
EPD for the best environmental decision 9
System boundaries (X=included, MND= module not declared, MNR=module not
relevant)
Benefits
& loads
Assembly
Product stage Use stage End of life stage beoyond
stage
system
boundary
EPD for the best environmental decision 10
slairetam
waR
tropsnarT
gnirutcafunaM
tropsnarT ylbmessA
esU
ecnanetniaM
riapeR
tnemecalpeR tnemhsibrufeR
esu
ygrene
lanoitarepO
esu
retaw
lanoitarepO
noitilomed
noitcurtsnoc-eD
tropsnarT
gnissecorp
etsaW
lasopsiD
-gnilcyceR-yrevoceR-esueR
laitnetop
LCA: Results
A1 A2 A3 A4 A5 B1 B2 B3 B4 B5 B6 B7 C1 C2 C3 C4 D
X X X X MND MND MND MND MND MND MND MND X X X X X
To ensure transparency for potential user of the product and in accordance with PSR-0011, the
table of environmental impacts represents the environmental impact of the functional unit, i.e.
the emission of 1 kW heating power.
The EPD was drawn up on the basis of 1 kW of heating power being supplied. The impact of the
stages of the life cycle of an installed product is calculated by the user of the declaration by
multiplying the impact concerned by the total heating capacity.
Core environmental impact indicators
Indicator Unit A1 A2 A3 A4 C1 C2 C3 C4 D
GWP-total kg CO2 eq. 2,7E+01 3,4E+00 6,7E+00 1,4E+00 0,0E+00 2,4E-01 4,8E-02 6,9E-04 -1,6E+01
GWP-fossil kg CO2 eq. 2,7E+01 3,4E+00 8,2E+00 1,4E+00 0,0E+00 2,4E-01 4,8E-02 6,7E-04 -1,6E+01
GWP-biogenic kg CO2 eq. 2,8E-01 1,1E-03 -1,6E+00 4,0E-04 0,0E+00 7,6E-05 4,6E-04 3,7E-06 8,2E-02
GWP-luluc kg CO2 eq. 3,3E-02 2,7E-05 9,6E-03 1,6E-05 0,0E+00 1,9E-06 9,8E-05 1,0E-08 3,2E-03
ODP kg CFC11 eq. 1,6E-06 8,0E-07 1,1E-06 3,1E-07 0,0E+00 5,7E-08 1,8E-09 1,5E-10 -5,2E-07
AP mol H+ eq. 1,3E-01 6,7E-03 3,3E-02 2,3E-02 0,0E+00 4,8E-04 2,4E-04 4,7E-06 -4,7E-02
EP-freshwater kg P eq. 1,1E-02 1,4E-05 1,2E-03 5,9E-06 0,0E+00 9,8E-07 2,2E-05 1,9E-06 -7,0E-03
EP-marine kg N eq. 3,5E-02 1,1E-03 7,3E-03 5,5E-03 0,0E+00 7,9E-05 4,9E-05 2,0E-06 -1,2E-02
EP-terrestrial mol N eq. 2,3E-01 1,2E-02 7,0E-02 6,1E-02 0,0E+00 8,8E-04 4,9E-04 2,2E-05 -1,3E-01
POCP kg NMVOC eq. 9,7E-02 4,4E-03 2,3E-02 1,6E-02 0,0E+00 3,1E-04 1,3E-04 6,5E-06 -8,5E-02
ADP-min. & met. kg Sb eq. 3,6E-05 1,5E-07 4,3E-06 4,1E-08 0,0E+00 1,0E-08 1,4E-09 3,0E-11 -8,5E-07
ADP-fossil MJ 3,1E+02 4,8E+01 1,4E+02 1,9E+01 0,0E+00 3,4E+00 6,2E-01 9,2E-03 -1,2E+02
WDP m3 1,5E+01 -8,0E-03 2,0E+00 -3,3E-03 0,0E+00 -5,7E-04 7,3E-03 -3,4E-03 -1,2E+00
GWP-total: Global Warming Potential; GWP-fossil: Global Warming Potential fossil fuels; GWP-biogenic: Global Warming Potential biogenic; GWP-LULUC:
Global Warming Potential land use and land use change; ODP: Depletion potential of the stratospheric ozone layer; AP: Acidification potential, Accumulated
Exceedance; EP-freshwater: Eutrophication potential, fraction of nutrients reaching freshwater end compartment; See “additional Norwegian requirements”
for indicator given as PO4 eq. EP-marine: Eutrophication potential, fraction of nutrients reaching freshwater end compartment; EP-terrestial: Eutrophication
potential, Accumulated Exceedance; POCP: Formation potential of tropospheric ozone; ADP-M&M: Abiotic depletion potential for non-fossil resources (minerals
and metals); ADP-fossil: Abiotic depletion potential for fossil resources; WDP: Water deprivation potential, deprivation weighted water counsumption
EPD for the best environmental decision 11
Additional environmental impact indicators
Indicator Unit A1 A2 A3 A4 C1 C2 C3 C4 D
PM Disease inc. 2,4E-06 2,3E-07 3,9E-07 8,8E-08 0,0E+00 1,6E-08 2,1E-09 3,6E-10 -8,2E-07
IRP kBq U-235 eq 2,2E+00 2,1E-01 6,6E-01 8,4E-02 0,0E+00 1,5E-02 6,9E-03 4,0E-05 1,2E+00
ETP-fw CTUe 8,1E+02 1,9E+01 5,6E+01 7,4E+00 0,0E+00 1,4E+00 6,6E-01 6,0E-02 -4,2E+02
HTP-c CTUh 3,9E-07 2,5E-10 1,1E-08 1,6E-10 0,0E+00 1,8E-11 7,5E-12 2,7E-12 2,3E-07
HTP-nc CTUh 1,8E-06 3,0E-08 4,2E-08 1,1E-08 0,0E+00 2,1E-09 3,7E-10 3,0E-11 -3,0E-07
SQP Pt 3,9E+01 1,3E-01 1,8E+02 5,0E-02 0,0E+00 9,2E-03 5,4E-02 1,5E-02 -8,9E+00
PM: Particulate matter emissions; IRP: Ionising radiation, human health; ETP-fw: Ecotoxicity (freshwater); ETP-c: Human toxicity, cancer effects; HTP-nc:
Human toxicity, non-cancer effects; SQP: Land use related impacts / soil quality
EPD for the best environmental decision 12
Classification of disclaimers to the declaration of core and additional environmental
impact indicators
ILCD
Indicator Disclaimer
classification
Global warming potential (GWP) None
ILCD type /
Depletion potential of the stratospheric ozone layer (ODP) None
level 1
Potential incidence of disease due to PM emissions (PM) None
Acidification potential, Accumulated Exceedance (AP) None
Eutrophication potential, Fraction of nutrients reaching freshwater end
None
compartment (EP-freshwater)
Eutrophication potential, Fraction of nutrients reaching marine end compartment
ILCD type / None
(EP-marine)
level 2
Eutrophication potential, Accumulated Exceedance (EP-terrestrial) None
Formation potential of tropospheric ozone (POCP) None
Potential Human exposure efficiency relative to U235 (IRP) 1
Abiotic depletion potential for non-fossil resources (ADP-minerals&metals) 2
Abiotic depletion potential for fossil resources (ADP-fossil) 2
Water (user) deprivation potential, deprivation-weighted water consumption
2
(WDP)
ILCD type /
Potential Comparative Toxic Unit for ecosystems (ETP-fw) 2
level 3
Potential Comparative Toxic Unit for humans (HTP-c) 2
Potential Comparative Toxic Unit for humans (HTP-nc) 2
Potential Soil quality index (SQP) 2
Disclaimer 1 – This impact category deals mainly with the eventual impact of low dose ionizing radiation on
human health of the nuclear fuel cycle. It does not consider effects due to
possible nuclear accidents, occupational exposure nor due to radioactive waste disposal in underground facilities.
Potential ionizing radiation from the soil, from radon and from some
construction materials is also not measured by this indicator.
Disclaimer 2 – The results of this environmental impact indicator shall be used with care as the uncertainties on
these results are high or as there is limited experienced with the indicator
EPD for the best environmental decision 13
Resource use
Indicator Unit A1 A2 A3 A4 C1 C2 C3 C4 D
RPEE MJ 1,8E+01 5,5E-02 1,7E+01 2,1E-02 0,0E+00 3,9E-03 6,9E-02 1,3E-05 6,4E+00
RPEM MJ 3,4E+00 1,8E-02 3,4E+01 6,9E-03 0,0E+00 1,3E-03 7,0E-03 4,5E-06 1,0E+00
TPE MJ 2,2E+01 7,3E-02 5,0E+01 2,7E-02 0,0E+00 5,2E-03 7,6E-02 1,7E-05 7,5E+00
NRPE MJ 3,1E+02 4,8E+01 1,4E+02 1,9E+01 0,0E+00 3,4E+00 6,2E-01 9,2E-03 -1,2E+02
NRPM MJ 4,4E-02 2,0E-05 7,9E-03 3,4E-05 0,0E+00 1,4E-06 2,3E-05 2,1E-08 -5,5E-03
TRPE MJ 3,1E+02 4,8E+01 1,4E+02 1,9E+01 0,0E+00 3,4E+00 6,2E-01 9,2E-03 -1,2E+02
SM kg 1,3E+01 0,0E+00 0,0E+00 0,0E+00 0,0E+00 0,0E+00 0,0E+00 0,0E+00 0,0E+00
RSF MJ 0,0E+00 0,0E+00 0,0E+00 0,0E+00 0,0E+00 0,0E+00 0,0E+00 0,0E+00 0,0E+00
NRSF MJ 0,0E+00 0,0E+00 0,0E+00 0,0E+00 0,0E+00 0,0E+00 0,0E+00 0,0E+00 0,0E+00
W m3 4,4E-01 1,2E-04 6,0E-02 5,4E-05 0,0E+00 8,7E-06 2,6E-04 -7,9E-05 -5,9E-02
RPEE Renewable primary energy resources used as energy carrier; RPEM Renewable primary energy resources used as raw materials; TPE Total use of
renewable primary energy resources; NRPE Non renewable primary energy resources used as energy carrier; NRPM Non renewable primary energy resources
used as materials; TRPE Total use of non renewable primary energy resources; SM Use of secondary materials; RSF Use of renewable secondary fuels; NRSF Use
of non renewable secondary fuels; W Use of net fresh water
End of life – Waste
Indicator Unit A1 A2 A3 A4 C1 C2 C3 C4 D
HW kg 1,0E-03 1,3E-04 1,4E-04 3,4E-05 0,0E+00 8,9E-06 2,2E-07 2,4E-08 -2,1E-03
NHW kg 8,9E+00 2,0E-03 2,3E-01 8,3E-04 0,0E+00 1,4E-04 2,0E-03 6,2E-07 2,4E+00
RW kg 8,7E-04 3,4E-04 3,2E-04 1,4E-04 0,0E+00 2,4E-05 2,0E-06 6,5E-08 2,4E-04
HW Hazardous waste disposed; NHW Non hazardous waste disposed; RW Radioactive waste disposed
EPD for the best environmental decision 14
End of life – output flow
Indicator Unit A1 A2 A3 A4 C1 C2 C3 C4 D
CR kg 0,0E+00 0,0E+00 0,0E+00 0,0E+00 0,0E+00 0,0E+00 0,0E+00 0,0E+00 0,0E+00
MR kg 0,0E+00 0,0E+00 1,2E+00 0,0E+00 0,0E+00 0,0E+00 1,8E+01 8,4E-02 0,0E+00
MER kg 0,0E+00 0,0E+00 0,0E+00 0,0E+00 0,0E+00 0,0E+00 0,0E+00 0,0E+00 0,0E+00
EEE MJ 0,0E+00 0,0E+00 0,0E+00 0,0E+00 0,0E+00 0,0E+00 0,0E+00 0,0E+00 0,0E+00
ETE MJ 0,0E+00 0,0E+00 0,0E+00 0,0E+00 0,0E+00 0,0E+00 0,0E+00 0,0E+00 0,0E+00
CR Components for reuse; MR Materials for recycling; MER Materials for energy recovery; EEE Exported electric energy; ETE Exported thermal energy
Information describing the biogenic carbon content at the factory gate
Biogenic carbon content Unit Value
Biogenic carbon content in product kg C 0,0E+00
Biogenic carbon content in the accompanying packaging kg C 4,5E-01
EPD for the best environmental decision 15
Additional Norwegian requirements
Greenhouse gas emission from the use of electricity in the manufacturing phase
National production mix from import, medium voltage (production of transmission lines, in
addition to direct emissions and losses in grid) of applied electricity for the manufacturing
prosess (A3). 23% of consumed electricity is provided by manufacturer’s solar panel park on the
roof of the factory. Therefore, emission factor acquired from Ecoinvent v3.8, representing Latvian
electricity mix (0.555 kgCO eq/kWh), has been recalculated to represent emission factor that is
2
specific to manufacturing plant and has solar power share included in it:
National electricity grid Unit Value
Weighted value, considering 23% share of solar panel system generation kg CO2 -eq/kWh 0,427
Additional environmental impact indicators required in NPCR Part A for construction
products
EP-freshwater is also declared in different units - PO 3- eq.
4
Indicator Unit A1 A2 A3 A4 C1 C2 C3 C4 D
EP- kg PO4
3,5E-02 4,2E-05 3,7E-03 1,8E-05 0,0E+00 3,0E-06 6,6E-05 5,8E-06 -2,1E-02
freshwater* eq.
EP-freshwater* Eutrophication potential, fraction of nutrients reaching freshwater end compartment.
Declared as PO 43- eq.
In order to increase the transparency of biogenic carbon contribution to climate impact, the
indicator GWP-IOBC is required as it declares climate impacts calculated according to the
principle of instantaneous oxidation. GWP-IOBC is also referred to as GWP-GHG in context of
Swedish public procurement legislation.
Indicator Unit A1 A2 A3 A4 C1 C2 C3 C4 D
GWP-IOBC kg CO2 eq. 2,6E+01 3,3E+00 8,1E+00 1,4E+00 0,0E+00 2,4E-01 4,7E-02 6,5E-04 -1,5E+01
GWP-IOBC global warming potential calculated according to the principle of instantaneous oxidation.
Hazardous substances
The declaration is based upon reference to threshold values and/or test results and/or material
safety data sheets provided to EPD verifiers. Documentation available upon request to EPD
owner.
⊠ The product contains no substances given by the REACH Candidate list or the Norwegian
priority list.
□ The product contains substances given by the REACH Candidate list or the Norwegian
priority list that are less than 0,1 % by weight.
□ The product contain dangerous substances, more then 0,1% by weight, given by the
REACH Candidate List or the Norwegian Priority list, see table.
□ The product contains no substances given by the REACH Candidate list or the Norwegian
priority list. The product is classified as hazardous waste (Avfallsforskiften, Annex III), see
table.
EPD for the best environmental decision 16
Indoor environment
The product meets the requirements for low emissions.
Carbon footprint
Carbon footprint has not been worked out for the product.
Bibliography
ISO 14025:2010 Environmental labels and declarations - Type III
environmental declarations - Principles and procedures
ISO 14040:2006 Environmental management – Life cycle assessment –
Principles and framework
ISO 14044:2006 Environmental management - Life cycle assessment -
Requirements and guidelines
EN 15804:2012+A2:2019 Sustainability of construction works - Environmental
product declaration - Core rules for the product category of
construction products
PCR-ed3-EN-2015 04 02 PCR Product Category Rules for Electrical, Electronic and
HVAC-R Products by PEP ecopassport® PROGRAM
PSR-0011-ed1.0-EN-2018 02 09 PSR specific rules for hot water radiators or towel radiators
by PEP ecopassport® PROGRAM
LCA software SimaPro 9.4
EPD-Norge GPI The Norwegian EPD Foundation/EPD-Norge, General
Programme Instructions 2019. Version 3.0 dated
2019.04.24
Program Operator tlf +47 23 08 80 00
The Norwegian EPD Foundation
Post Box 5250 Majorstuen, 0303
e-post: post@epd-norge.no
Oslo
Norway web www.epd-norge.no
Publisher tlf +47 23 08 80 00
The Norwegian EPD Foundation
Post Box 5250 Majorstuen, 0303
e-post: post@epd-norge.no
Oslo
Norway web www.epd-norge.no
Owner of the declaration tlf +371 67 79 67 10
Lyngson SIA
"Akači", Grēnes, Olaines novads e-post: info@lyngson.lv
Latvia web lyngson.lv
Author of the life cycle assesment tlf +371 67 25 68 29
Bureau Veritas Latvia
Duntes iela 17A, Rīga e-post: riga@bureauveritas.com
Latvia web bureauveritas.lv
EPD for the best environmental decision 17
EPD for the best
environmental
decision
EPD for the best environmental decision 18
