Environmental Product
Declaration
In accordance with ISO 14025 and EN 15804 +A2
Owner of the declaration: SiTech+ PP Pipe STEM
Norsk Wavin AS
Program holder and publisher:
Wavin SiTech+ is a waste water
The Norwegian EPD foundation
system made of mineral-
reinforced polypropylene (PP),
Declaration number: which offers increased durability,
NEPD-3475-2069-EN
but more importantly is quiet and
easy to install.
Registration Number:
NEPD-3475-2069-EN
Manufacturer
Issue date: 27.05.2022
Wavin Germany Twist
Valid to: 27.05.2027
The Norwegian EPD Foundation Ver2-101122
General information
Product: Owner of the declaration:
SiTech+ PP Pipe STEM with socket Norsk Wavin AS
Contact person: Matteo Tagliaferri
Program Operator: Phone: +31 623193684
e-mail: matteo.tagliaferri@wavin.com
The Norwegian EPD Foundation
Post Box 5250 Majorstuen, 0303 Oslo, Norway
Tlf: +47 23 08 80 00 Manufacturer:
e-mail: post@epd-norge.no Wavin Germany Twist
Industriestraße 20, 49767, Twist, Germany
Declaration Number: Phone: +49 5936 12 0
e-mail: info@wavin.de
NEPD-3475-2069-EN
Place of production:
This declaration is based on Product
Industriestraße 20, 49767, Twist, Germany
Category Rules:
CEN standard EN 15804:2012+A2:2019 serves as
Management system:
core PCR, supplied with NPCR Part A, Version 2.0.
EN ISO 9001:2015 and EN ISO 14001:2015
Statements:
Organization no:
The owner of the declaration shall be liable for the
underlying information and evidence. EPD 823355092
Norway shall not be liable with respect to
manufacturer, life cycle assessment data and Issue date:
evidences. 27.05.2022
Declared unit: Valid to:
1 kg SiTech+ Pipe STEM 110 27.05.2027
Declared unit with option: Year of study:
A1,A2,A3,A4,A5,C1,C2,C3,C4,D 2020
Functional unit: Comparability:
Not applicable. EPDs from other programmes than the Norwegian
EPD foundation may not be comparable.
Verification:
Independent verification of the declaration and
The EPD has been worked out by:
data, according to ISO14025:2010
Lisa Overmars and Emma Thunnissen,
internal external Ecochain Technologies
Harry van Ewijk, SGS Search
Approved (Manager of EPD Norway)
Independent verifier approved by EPD Norway
EPD for the best environmental decision 2
Product
Product description:
Wavin SiTech+ is a low-noise soil & waste drainage system. The 3-layer pipe structure reduces
noise levels, while the use of mineral reinforced polypropylene (PP) results in a high durability
and heat-resistance. Wavin SiTech+ meets all standards set for soil & waste discharge systems
(EN 1451-1), including noise reduction and fire resistance standards (EN 13501-1). The
socketed connections and prefabricated elastomer gaskets (SBR) enable fast, easy and secure
installation. The covered products are described in the Technical Data section.
Product specification:
A typical composition of the pipes, including packaging, covered in this EPD is as follows:
Materials %
PP 53%
Filler 32%
Additives 1%
Rubber gasket 1%
Packaging 14%
The physical properties of the pipes covered in this EPD are:
• Fire behavior: Class C-s2, d0 according to EN13501-1.
• Density ~ 1,3 gr/cm3
• Working Temperature: 90°C continuous temperature; 95°C peak temperature.
• Linear coefficient of thermal expansion ~ 0,12 mm/mK.
• Impact Test -20°C according to EN744.
• Ring Stiffness > = 5,5 Kn/m2 (ref. OD110)
The color of the pipe is black (BK).
Technical data:
The declared unit of this EPD is 1 kg SiTech+ Pipe STEM 110. The results per kg are based on
the product ‘SiTech+ Pipe STEM 110 L=2 S/PL NP’ (‘base product’). The Table below provides
the products covered with this EPD. The selected base product is representative for all products
described in this Table; deviations of the LCA results of the other products compared to the base
product are not more than 10%. The list below provides the mass per 1 meter pipe (including
packaging). These masses should be used to calculate the LCA results per 1 meter pipe, by
multiplying the results presented on page 7-10 with the weights specified below.
Mass Mass
Product Product
(kg/meter) (kg/meter)
SiTech+ PP Pipe STEM BK 110 L=0,5 S/PL 1.98 SiTech+ Pipe STEM 110 L=0,5 S/PL NP 1.84
SiTech+ PP Pipe STEM BK 110 L=1 S/PL 1.76 SiTech+ Pipe STEM 110 L=1 S/PL NP 2.19
SiTech+ PP Pipe STEM BK 110 L=2 S/PL 1.65 SiTech+ Pipe STEM 110 L=2 S/PL NP 1.87
SiTech+ PP Pipe STEM BK 110 L=3 S/PL 1.61 SiTech+ Pipe STEM 110 L=3 S/PL NP 1.76
EPD for the best environmental decision 3
Market:
Europe, but the EPD is specific for Nordic countries.
Reference service life, product:
Lifetime on product calculated more than 100 year
Reference service life, building:
LCA: Calculation rules
Declared unit:
1 kg SiTech+ Pipe STEM 110
Data quality:
For module A1, specific data for product compositions as provided by the manufacturer are
used. For module A2, transportation data of the raw materials used to the production site was
collected. For module A3, energy consumption and waste production data was collected for
production year 2020. The used background processes are derived from Ecoinvent 3.6.
Allocation:
Allocation was carried out in accordance with the provisions of the EN15804. All manufacturing
inputs (energy and auxiliary materials) at production site level are allocated to different
production processes, followed by allocation of the production processes to the products that
are produced using these processes through mass allocation. No secondary materials have been
used in the production process.
System boundary:
Modules A1-A5 and C1-D are included. The figure below shows a (simplified) process tree.
EPD for the best environmental decision 4
Cut-off criteria:
All relevant inputs and outputs - like emissions, energy and materials - have been taken into
account in this LCA. In accordance with EN15804, the total neglected input flows per module
does not exceed 5% of energy usage and mass
LCA: Scenarios and additional technical information
The following information describe the scenarios in the different modules of the EPD.
Transport from production place to assembly/user (A4)
The transportation distance from Twist to Oslo was considered.
Capacity utilisation
Type Type of vehicle Distance KM Fuel/Energy consumption
(incl. return) %
Truck 50% Unspecified 945 0,027 l diesel/tkm
Boat 50% Ferry 163 0,0295 kg heavy fuel oil/tkm
EPD for the best environmental decision 5
Assembly (A5)
Product losses of 10% are considered. The installation is done manually, and therefore no
energy is needed.
Unit Value
Material loss kg 0,1
Packaging waste kg 0,14
End of Life (C1, C3, C4)
Demolition is done manually, and therefore no energy is needed. The considered waste
treatment for the pipe is 70% recycling, 20% incineration with energy recovery and 10%
landfill. The considered waste treatment for the rubber gasket is 85% incineration with energy
recovery, 10% landfill, and 5% recycling. The amount ‘collected as mixed construction waste’ is
based on the 1 kg, minus the amount of packaging waste.
Unit Value
Collected as mixed construction waste kg 0,86
Reuse kg 0
Recycling kg 0,60
Energy recovery kg 0,18
To landfill kg 0,09
Transport to waste processing (C2)
The considered distances are 50 km to landfill, 100 km for energy recovery, and 250 km for
recycling.
Capacity utilisation
Type Type of vehicle Distance KM Fuel/Energy consumption
(incl. return) %
Truck 50% Unspecified 199,4 0,027 l diesel/tkm
Benefits and loads beyond the system boundaries (D)
For the PP, and additives, 0,67 kg of saved virgin PP was considered per kg material recycled
(total of A5 en C3). For the filler, 0,67 kg of saved virgin filler was considered per kg filler
recycled. The benefits from exported energy were calculation from the energy efficiencies for
Northern countries reported by CEWEP, which is equal to an electrical efficiency of 11,0%, and
a thermal efficiency of 72,6%. Energy recovery from all materials (including rubber gasket and
packaging) was considered. Substition of Norwegian electricity mix and district heating mix was
assumed.
Unit Value
Saving of virgin PP kg 0,28
Saving of virgin filler kg 0,16
Substition of electric energy MJ 0,62
Subsitition of thermal energy MJ 4,12
EPD for the best environmental decision 6
Additional technical information
Not applicable.
LCA: Results
The LCA results are presented below for the declared unit defined on page 2 of the EPD
document. Recalculation to results for pipes per meter can be done based on the technical data
specified on page 3.
System boundaries (X=included, MND= module not declared, MNR=module not
relevant)
Benefits
& loads
Assembly
Product stage Use stage End of life stage beyond
stage
system
boundary
n -
s la ir e wt a am R t r o p s n a r T g n ir u t c a fu n a M t r o p s n a r T y lb m e s s A e s U e c n a n e t n ia M r ia p e R t n e m e c a lp e R t n e m h s ib r u fe R la n o ity ag rr eee pns Ou e la n o it ar re ete a ps w Ou n o io t cit ui rlo t sm ne od
c
-
t r o p s n a r T g n is s ee tc so ar Wp la s o p s iD g yn r eil v ec soy uc ce e RR --la it n e t o p
e e
D R
A1 A2 A3 A4 A5 B1 B2 B3 B4 B5 B6 B7 C1 C2 C3 C4 D
X X X X X X X X X X
Core environmental impact indicators
Indicator Unit A1-A3 A4 A5 C1 C2 C3 C4 D
GWP-total kg CO2 eq. 8,10E-01 1,22E-01 6,79E-01 0,00E+00 2,27E-02 5,10E-01 6,89E-03 -8,17E-01
GWP-fossil kg CO2 eq. 1,28E+00 1,22E-01 1,98E-01 0,00E+00 2,27E-02 5,11E-01 6,89E-03 -8,15E-01
GWP-biogenic kg CO2 eq. -4,68E-01 6,12E-05 4,81E-01 0,00E+00 1,38E-05 -7,62E-04 6,33E-06 -2,63E-03
GWP-LULUC kg CO2 eq. 3,67E-03 4,72E-05 3,87E-04 0,00E+00 8,02E-06 1,27E-04 1,42E-07 -2,55E-04
ODP kg CFC11 eq. 5,11E-08 2,76E-08 1,08E-08 0,00E+00 5,22E-09 1,67E-08 2,36E-10 -4,36E-08
AP mol H⁺ eq. 5,06E-03 1,11E-03 7,51E-04 0,00E+00 1,29E-04 6,82E-04 5,37E-06 -2,40E-03
EP-freshwater kg P eq. 2,19E-05 9,35E-07 2,72E-06 0,00E+00 1,86E-07 3,66E-06 6,29E-09 -9,39E-06
EP-marine kg N eq. 9,87E-04 3,42E-04 1,80E-04 0,00E+00 4,62E-05 1,95E-04 3,19E-06 -4,59E-04
EP-terrestial mol N eq. 1,12E-02 3,78E-03 2,03E-03 0,00E+00 5,09E-04 2,14E-03 2,19E-05 -5,46E-03
kg NMVOC
POCP 4,47E-03 1,04E-03 7,04E-04 0,00E+00 1,45E-04 6,83E-04 7,73E-06 -2,15E-03
eq.
ADP-M&M kg Sb eq. 2,49E-05 3,18E-06 3,26E-06 0,00E+00 6,52E-07 3,07E-06 5,87E-09 -5,83E-06
ADP-fossil MJ 4,16E+01 1,83E+00 4,66E+00 0,00E+00 3,48E-01 2,22E+00 1,68E-02 -2,42E+01
WDP m³ 1,19E+00 5,28E-03 1,24E-01 0,00E+00 1,07E-03 4,27E-02 7,51E-05 -4,07E-01
EPD for the best environmental decision 7
GWP-total: Global Warming Potential; GWP-fossil: Global Warming Potential fossil fuels; GWP-biogenic:
Global Warming Potential biogenic; GWP-LULUC: Global Warming Potential land use and land use change;
ODP: Depletion potential of the stratospheric ozone layer; AP: Acidification potential, Accumulated
Exceedance; EP-freshwater: Eutrophication potential, fraction of nutrients reaching freshwater end
compartment; See “additional Norwegian requirements” for indicator given as PO4 eq. EP-marine:
Eutrophication potential, fraction of nutrients reaching freshwater end compartment; EP-terrestial:
Eutrophication potential, Accumulated Exceedance; POCP: Formation potential of tropospheric ozone; ADP-
M&M: Abiotic depletion potential for non-fossil resources (minerals and metals); ADP-fossil: Abiotic
depletion potential for fossil resources; WDP: Water deprivation potential, deprivation weighted water
counsumption
Additional environmental impact indicators
Indicator Unit A1-A3 A4 A5 C1 C2 C3 C4 D
Disease
PM 6,78E-08 1,01E-08 9,68E-09 0,00E+00 2,05E-09 1,15E-08 1,13E-10 -2,20E-08
incidence
kBq U235
IRP 3,11E-02 7,99E-03 4,96E-03 0,00E+00 1,52E-03 6,69E-03 7,65E-05 -1,25E-02
eq.
ETP-fw CTUe 1,06E+01 1,45E+00 1,54E+00 0,00E+00 2,82E-01 2,49E+00 1,29E-02 -5,61E+00
HTP-c CTUh 4,92E-10 5,53E-11 1,20E-10 0,00E+00 1,00E-11 2,77E-10 3,53E-13 -1,66E-10
HTP-nc CTUh 1,06E-08 1,68E-09 1,77E-09 0,00E+00 3,37E-10 3,57E-09 8,03E-12 -4,58E-09
Dimensionle
SQP 4,58E+01 1,42E+00 4,98E+00 0,00E+00 2,98E-01 1,79E+00 4,14E-02 -1,19E+01
ss
PM: Particulate matter emissions; IRP: Ionising radiation, human health; ETP-fw: Ecotoxicity (freshwater);
ETP-c: Human toxicity, cancer effects; HTP-nc: Human toxicity, non-cancer effects; SQP: Land use related
impacts / soil quality
Classification of disclaimers to the declaration of core and additional environmental
impact indicators
ILCD
Indicator Disclaimer
classification
Global warming potential (GWP) None
ILCD type / level
Depletion potential of the stratospheric ozone layer (ODP) None
1
Potential incidence of disease due to PM emissions (PM) None
Acidification potential, Accumulated Exceedance (AP) None
Eutrophication potential, Fraction of nutrients reaching freshwater end
None
compartment (EP-freshwater)
Eutrophication potential, Fraction of nutrients reaching marine end
None
ILCD type / level compartment (EP-marine)
2
Eutrophication potential, Accumulated Exceedance (EP-terrestrial) None
Formation potential of tropospheric ozone (POCP) None
Potential Human exposure efficiency relative to U235 (IRP) 1
Abiotic depletion potential for non-fossil resources (ADP-minerals&metals) 2
Abiotic depletion potential for fossil resources (ADP-fossil) 2
ILCD type / level Water (user) deprivation potential, deprivation-weighted water consumption
2
3 (WDP)
Potential Comparative Toxic Unit for ecosystems (ETP-fw) 2
Potential Comparative Toxic Unit for humans (HTP-c) 2
EPD for the best environmental decision 8
Potential Comparative Toxic Unit for humans (HTP-nc) 2
Potential Soil quality index (SQP) 2
Disclaimer 1 – This impact category deals mainly with the eventual impact of low dose ionizing radiation on
human health of the nuclear fuel cycle. It does not consider effects due to
possible nuclear accidents, occupational exposure nor due to radioactive waste disposal in underground facilities.
Potential ionizing radiation from the soil, from radon and from some
construction materials is also not measured by this indicator.
Disclaimer 2 – The results of this environmental impact indicator shall be used with care as the uncertainties on
these results are high or as there is limited experienced with the indicator
Resource use
Parameter Unit A1-A3 A4 A5 C1 C2 C3 C4 D
RPEE MJ 8,81E+00 2,47E-02 8,96E-01 0,00E+00 4,99E-03 1,09E-01 5,48E-04 -2,56E+00
RPEM MJ 0,00E+00 0,00E+00 0,00E+00 0,00E+00 0,00E+00 0,00E+00 0,00E+00 0,00E+00
TPE MJ 8,81E+00 2,47E-02 8,96E-01 0,00E+00 4,99E-03 1,09E-01 5,48E-04 -2,56E+00
NRPE MJ 4,47E+01 1,94E+00 4,99E+00 0,00E+00 3,69E-01 2,36E+00 1,78E-02 -2,62E+01
NRPM MJ 0,00E+00 0,00E+00 0,00E+00 0,00E+00 0,00E+00 0,00E+00 0,00E+00 0,00E+00
TRPE MJ 4,47E+01 1,94E+00 4,99E+00 0,00E+00 3,69E-01 2,36E+00 1,78E-02 -2,62E+01
SM kg 0,00E+00 0,00E+00 0,00E+00 0,00E+00 0,00E+00 0,00E+00 0,00E+00 0,00E+00
RSF MJ 0,00E+00 0,00E+00 0,00E+00 0,00E+00 0,00E+00 0,00E+00 0,00E+00 0,00E+00
NRSF MJ 0,00E+00 0,00E+00 0,00E+00 0,00E+00 0,00E+00 0,00E+00 0,00E+00 0,00E+00
W m3 2,18E-02 1,94E-04 2,39E-03 0,00E+00 3,94E-05 1,25E-03 2,05E-05 -6,19E-03
RPEE Renewable primary energy resources used as energy carrier; RPEM Renewable primary energy
resources used as raw materials; TPE Total use of renewable primary energy resources; NRPE Non
renewable primary energy resources used as energy carrier; NRPM Non renewable primary energy
resources used as materials; TRPE Total use of non renewable primary energy resources; SM Use of
secondary materials; RSF Use of renewable secondary fuels; NRSF Use of non renewable secondary fuels; W
Use of net fresh water
End of life - Waste
Parameter Unit A1-A3 A4 A5 C1 C2 C3 C4 D
HW KG 1,08E-05 4,35E-06 2,09E-06 0,00E+00 8,89E-07 3,58E-06 1,98E-08 -7,37E-06
NHW KG 1,14E-01 1,02E-01 5,37E-02 0,00E+00 2,16E-02 1,08E-01 8,64E-02 -2,28E-02
RW KG 3,16E-05 1,25E-05 5,81E-06 0,00E+00 2,37E-06 8,50E-06 1,11E-07 -1,19E-05
HW Hazardous waste disposed; NHW Non hazardous waste disposed; RW Radioactive waste disposed
End of life – output flow
Parameter Unit A1-A3 A4 A5 C1 C2 C3 C4 D
CR kg 0,00E+00 0,00E+00 7,48E-03 0,00E+00 0,00E+00 0,00E+00 0,00E+00 0,00E+00
MR kg 0,00E+00 0,00E+00 7,48E-02 0,00E+00 0,00E+00 5,99E-01 0,00E+00 0,00E+00
MER kg 0,00E+00 0,00E+00 1,38E-01 0,00E+00 0,00E+00 1,76E-01 0,00E+00 0,00E+00
EEE MJ 0,00E+00 0,00E+00 0,00E+00 0,00E+00 0,00E+00 0,00E+00 0,00E+00 6,26E-01
EPD for the best environmental decision 9
ETE MJ 0,00E+00 0,00E+00 0,00E+00 0,00E+00 0,00E+00 0,00E+00 0,00E+00 4,12E+00
CR Components for reuse; MR Materials for recycling; MER Materials for energy recovery; EEE Exported
electric energy; ETE Exported thermal energy
Information describing the biogenic carbon content at the factory gate
Biogenic carbon content Unit Value
Biogenic carbon content in product kg C 0
Biogenic carbon content in the accompanying packaging kg C 0,131
Additional Norwegian requirements
Greenhous gas emission from the use of electricity in the manufacturing phase
National production mix from import, low voltage (production of transmission lines, in addition
to direct emissions and losses in grid) of applied electricity for the manufacturing process(A3).
National electricity grid Unit Value
Hydroelectricity, average (Ecoinvent 3.6) kg CO2 -eq/kWh 0,0496
Additional environmental impact indicators required in NPCR Part A for construction
products
In order to increase the transparency of biogenic carbon contribution to climate impact, the
indicator for GWP has been sub-divided into the following:
GWP-IOBC Climate impacts calculated according to the principle of instantanious oxidation
GWP-BC Climate impacts from the net uptake and emission of biogenic carbon from each
module.
Indicator Unit A1-A3 A4 A5 C1 C2 C3 C4 D
GWP-IOBC kg CO2 eq. 1,28E+00 1,22E-01 1,98E-01 0,00E+00 2,27E-02 5,11E-01 6,88E-03 -8,15E-01
GWP-BC kg CO2 eq. -4,68E-01 6,12E-05 4,81E-01 0,00E+00 1,38E-05 -7,62E-04 6,33E-06 -2,63E-03
GWP kg CO2 eq. 8,10E-01 1,22E-01 6,79E-01 0,00E+00 2,27E-02 5,10E-01 6,89E-03 -8,17E-01
GWP-IOBC Global warming potential calculated according to the principle of instantanious oxidation. GWP-
BC Global warming potential from net uptake and emissions of biogenic carbon from the materials in each
module. GWP Global warming potential
Hazardous substances
The declaration is based upon reference to threshold values and/or test results and/or material
safety data sheets provided to EPD verifiers. Documentation available upon request to EPD
owner.
✓ The product contains no substances given by the REACH Candidate list or the
Norwegian priority list.
□ The product contains substances given by the REACH Candidate list or the Norwegian
priority list that are less than 0,1 % by weight.
EPD for the best environmental decision 10
□ The product contain dangerous substances, more then 0,1% by weight, given by the
REACH Candidate List or the Norwegian Priority list, see table.
□ The product contains no substances given by the REACH Candidate list or the
Norwegian priority list. The product is classified as hazardous waste (Avfallsforskiften,
Annex III), see table.
Indoor environment
The product meets the requirements for low emissions.
Carbon footprint
Carbon footprint has not been worked out for the product.
EPD for the best environmental decision 11
Bibliography
ISO 14025:2010 Environmental labels and declarations - Type III environmental
declarations - Principles and procedures
ISO 14044:2006 Environmental management - Life cycle assessment -
Requirements and guidelines
EN 15804:2012+A2:2019 Sustainability of construction works - Environmental product
declaration - Core rules for the product category of construction
products
ISO 21930:2007 Sustainability in building construction - Environmental
declaration of building products
NPCR Part A Construction products and services. Ver. 2.0. March 2021, EPD-
Norge
CEWEP Results of Specific Data for Energy, R1 Plant Efficiency Factor and
NCV of 314 European Waste-to-Energy (WtE) Plants, CEWEP
Energy Report III (status 2007-2010), 2012, Reiman, D.O.
Program Operator tlf +47 23 08 80 00
The Norwegian EPD Foundation
Post Box 5250 Majorstuen, 0303 Oslo e-post: post@epd-norge.no
Norway web www.epd-norge.no
Publisher tlf +47 23 08 80 00
The Norwegian EPD Foundation
Post Box 5250 Majorstuen, 0303 Oslo e-post: post@epd-norge.no
Norway web www.epd-norge.no
Owner of the declaration tlf +4745190625
Norsk Wavin AS Fax
Karihaugveien 89, 1086, Oslo e-post: Invoice.no@wavin.com
Norway web www.wavin.com/nn-no
Author of the life cycle assessment tlf +31 (0)20 303 5777
Lisa Overmars Fax
H.J.E. Wenckebachweg 123, 1096 AM
e-post: lovermars@ecochain.com
Amsterdam
The Netherlands web www.ecochain.com
EPD for the best environmental decision 12
EPD for the best
environmental
decision
The Norwegian EPD foundation
www.epd-norge.no
