Environmental product declaration
in accordance with ISO 14025 and EN 15804+A2
AXQJ 4x95/29-AS 0.6/1kV
OOwwnneerr ooff tthhee ddeeccllaarraattiioonn:: PPrrooggrraamm ooppeerraattoorr::
Amokabel AB The Norwegian EPD Foundation
PPrroodduucctt:: DDeeccllaarraattiioonn nnuummbbeerr::
AXQJ 4x95/29-AS 0.6/1kV NEPD-8382-7999-EN
DDeeccllaarreedd uunniitt:: RReeggiissttrraattiioonn nnuummbbeerr::
1 m NEPD-8382-7999-EN
TThhiiss ddeeccllaarraattiioonn iiss bbaasseedd oonn PPrroodduucctt CCaatteeggoorryy IIssssuuee ddaattee::
RRuulleess:: 06.12.2024
CEN Standard EN 15804:2012+A2:2019 serves as core
VVaalliidd ttoo::
The Norwegian EPD Foundation PCR
06.12.2029
NPCR 027:2020 Part B for Electrical cables and wires
EEPPDD ssooffttwwaarree::
LCAno EPD generator ID: 645244
1 / 12
GGeenneerraall iinnffoorrmmaattiioonn
PPrroodduucctt OOwwnneerr ooff tthhee ddeeccllaarraattiioonn::
AXQJ 4x95/29-AS 0.6/1kV Amokabel AB
Contact person: Oskar Wijk
Phone: +46 481-750 810
e-mail: oskar.wijk@amokabel.com
PPrrooggrraamm ooppeerraattoorr:: MMaannuuffaaccttuurreerr::
The Norwegian EPD Foundation Amokabel AB
Post Box 5250 Majorstuen, 0303 Oslo, Norway
Phone: +47 977 22 020
web: www.epd-norge.no
DDeeccllaarraattiioonn nnuummbbeerr:: PPllaaccee ooff pprroodduuccttiioonn::
Amokabel AB
NEPD-8382-7999-EN
Kabelvägen 5
SE-36443 Alstermo, Sweden
TThhiiss ddeeccllaarraattiioonn iiss bbaasseedd oonn PPrroodduucctt CCaatteeggoorryy RRuulleess:: MMaannaaggeemmeenntt ssyysstteemm::
CEN Standard EN 15804:2012+A2:2019 serves as core PCR ISO 14001, ISO 9001, ISO 45001
NPCR 027:2020 Part B for Electrical cables and wires
SSttaatteemmeenntt ooff lliiaabbiilliittyy:: OOrrggaanniissaattiioonn nnoo::
The owner of the declaration shall be liable for the underlying 556510-2471
information and evidence. EPD Norway shall not be liable with respect
to manufacturer information, life cycle assessment data and
evidences.​
DDeeccllaarreedd uunniitt:: IIssssuuee ddaattee::
1 m AXQJ 4x95/29-AS 0.6/1kV 06.12.2024
DDeeccllaarreedd uunniitt wwiitthh ooppttiioonn:: VVaalliidd ttoo::
A1,A2,A3,A4,A5,B1,B2,B3,B4,B5,B6,B7,C1,C2,C3,C4,D 06.12.2029
YYeeaarr ooff ssttuuddyy::
2023
FFuunnccttiioonnaall uunniitt:: CCoommppaarraabbiilliittyy::
1 m of AXQJ 4x95/29-AS 0.6/1kV installed electrical cables used to EPD of construction products may not be comparable if they not
transmit a reference electric current of 1A over a specific lifetime, comply with EN 15804 and seen in a building context.
including waste treatment at end-of-life.
GGeenneerraall iinnffoorrmmaattiioonn oonn vveerriiffiiccaattiioonn ooff EEPPDD ffrroomm EEPPDD ttoooollss:: DDeevveellooppmmeenntt aanndd vveerriiffiiccaattiioonn ooff EEPPDD::
Independent verification of data, other environmental information The declaration is created using EPD tool lca.tools ver EPD2022.03,
and the declaration according to ISO 14025:2010, § 8.1.3 and § 8.1.4. developed by LCA.no. The EPD tool is integrated in the company's
Verification of each EPD is made according to EPD-Norway’s management system, and has been approved by EPD Norway.
guidelines for verification and approval requiring that tools are i) Approval number:
integrated into the company's environmental management system, ii)
the procedures for use of the EPD tool are approved by EPD-Norway, Developer of EPD: Peter Eriksson
and iii) the process is reviewed annually by an independent third
Reviewer of company-specific input data and EPD:​ Oskar Wijk
party verifier. See Appendix G of EPD-Norway's General Programme
Instructions for further information on EPD tools
VVeerriiffiiccaattiioonn ooff EEPPDD ttooooll:: AApppprroovveedd::
Independent third party verification of the EPD tool, background data
and test-EPD in accordance with EPDNorway's procedures and
guidelines for verification and approval of EPD tools. Approval
number: NEPDT32.
Third party verifier:
Vito D’Incognito, Take Care International
(no signature required)
2 / 12
PPrroodduucctt
PPrroodduucctt ddeessccrriippttiioonn::
1 kV AXQJ is a halogen-free and flame-retardant cable, 0.6/1kV, suitable for open fixed installations both indoors and outdoors, in soil, air, water,
and in conduits. It features copper sector-shaped cores ranging from 50mm² to 300mm², and a screen of annealed copper wire with counter helix.
PPrroodduucctt ssppeecciiffiiccaattiioonn
MMaatteerriiaallss kkgg %%
Copper foil 0,01 0,56
HFFR Polyolefin 0,37 20,64
Metal - Copper 0,24 13,62
Plastic - Polyethylene 0,20 11,14
Metal - Aluminium 0,97 54,04
Total 1,79 100,00
PPaacckkaaggiinngg kkgg %%
Packaging - Wooden drums 0,36 100,00
Total incl. packaging 2,15 100,00
TTeecchhnniiccaall ddaattaa::
1Maximum Conductor Temperature: -20°C to +90°C
Voltage Rating U0/U: 0.6/1kV
Stranded, sector-shaped, annealed aluminum according to EN 60228 Class 2
MMaarrkkeett::
Sweden
RReeffeerreennccee sseerrvviiccee lliiffee,, pprroodduucctt
40 years
RReeffeerreennccee sseerrvviiccee lliiffee,, bbuuiillddiinngg oorr ccoonnssttrruuccttiioonn wwoorrkkss
40 years
LLCCAA:: CCaallccuullaattiioonn rruulleess
DDeeccllaarreedd uunniitt::
1 m AXQJ 4x95/29-AS 0.6/1kV
CCuutt--ooffff ccrriitteerriiaa::
All major raw materials and all the essential energy is included. The production processes for raw materials and energy flows with very small
amounts (less than 1%) are not included. These cut-off criteria do not apply for hazardous materials and substances.
AAllllooccaattiioonn::
The allocation is made in accordance with the provisions of EN 15804. Incoming energy and water and waste production in-house is allocated
equally among all products through mass allocation. Effects of primary production of recycled materials is allocated to the main product in which
the material was used. The recycling process and transportation of the material is allocated to this analysis.
DDaattaa qquuaalliittyy::
Specific data for the product composition are provided by the manufacturer. The data represent the production of the declared product and were
collected for EPD development in the year of study. Background data is based on EPDs according to EN 15804 and different LCA databases. The
data quality of the raw materials in A1 is presented in the table below.
MMaatteerriiaallss SSoouurrccee DDaattaa qquuaalliittyy YYeeaarr
Copper foil ecoinvent 3.6 Database 2019
HFFR Polyolefin Ecoinvent 3.6 Database 2019
Metal - Aluminium ecoinvent 3.6 Database 2019
Metal - Copper ecoinvent 3.6 Database 2019
Supplier data +
Packaging - Wooden drums Modified ecoinvent 3.6 2019
database
Plastic - Polyethylene ecoinvent 3.6 Database 2019
3 / 12
SSyysstteemm bboouunnddaarriieess ((XX==iinncclluuddeedd,, MMNNDD==mmoodduullee nnoott ddeeccllaarreedd,, MMNNRR==mmoodduullee nnoott rreelleevvaanntt))
CCoonnssttrruuccttiioonn BBeeyyoonndd tthhee ssyysstteemm
PPrroodduucctt ssttaaggee UUssee ssttaaggee EEnndd ooff lliiffee ssttaaggee
iinnssttaallllaattiioonn ssttaaggee bboouunnddaarriieess
A1 A2 A3 A4 A5 B1 B2 B3 B4 B5 B6 B7 C1 C2 C3 C4 D
X X X X X X X X X X X X X X X X X
SSyysstteemm bboouunnddaarryy::
The analysis is a cradle-to-grave study made for 1 m of cable manufactured , installed and used outdoor over the lifetime 40 years. Modules A1-
A5 are included in the analysis. It includes the extraction and production of raw materials, transportation to the factory, the production process
itself, transportation to market and installation of the product. Modules B1-B7 describe the use phase and are declared for an outdoor cable. B6 is
the operational energy usage based on a normal use. C1-C4, D are mandatory modules which include end of life treatment of materials and the
benefits from recycling.
The flowchart below illustrates the system boundaries of the analysis:
The flowchart below illustrates the system boundaries of the analysis:
AAddddiittiioonnaall tteecchhnniiccaall iinnffoorrmmaattiioonn::
The reference product AXQJ 4x95/29-AS 0.6/1kV represents the entire product family. Please contact us for a specific EPD of another cable in the
product family:
AXQJ 3x50/16-AS
AXQJ 4x50/16-AS
AXQJ 4x50/29-AS
AXQJ 3x70/21-AS
AXQJ 4x70/21-AS
AXQJ 3x95/29-AS
AXQJ 4x95/29-AS
AXQJ 4x95/57-AS
AXQJ 3x120/41-AS
AXQJ 4x120/41-AS
AXQJ 3x150/41-AS
AXQJ 4x150/41-AS
AXQJ 4x150/88-AS
AXQJ 3x185/57-AS
AXQJ 4x185/57-AS
AXQJ 3x240/72-AS
AXQJ 4x240/72-AS
AXQJ 4x240/146-AS
AXQJ 3x300/88-AS
AXQJ 4x300/88-AS
waR slairetam tropsnarT gnirutcafunaM tropsnarT ylbmessA e​sU ecnanetniaM riapeR tnemecalpeR tnemhsibrufeR lanoitarepO ygrene esu lanoitarepO esu retaw -eD noitcurtsnoc noitilomed tropsnarT etsaW gnissecorp lasopsiD -yrevoceR-esueR laitnetop-gnilcyceR
4 / 12
LLCCAA:: SScceennaarriiooss aanndd aaddddiittiioonnaall tteecchhnniiccaall iinnffoorrmmaattiioonn
The following information describe the scenarios in the different modules of the EPD.
Module A4 = The scenario considered in this EPD is based on true distansces from suppliers.
Modules A5 = 2 % product losses during installation are estimated by the company. No energy use for installation has been quantified since this
operation is assumed to be done with other products and should be assessed at a construction works level. Cable drums are reused and assumed
under the cut-off criterion of 1%.
For B1-B7 the default environmental impact and resource indicators in the EPD are assumed to be zero. Some other potential environmental
impacts from the use phase might not be covered by the scope of an EPD.
Module B6 = The operational energy use of the cable is calculated based on the methodology described in PEP Ecopassport, Product Specific Rules
(PSR) for wires, cables
and accessories, reference PSR-0001-ed3-EN-2015 10 16. The following parameters are used to calculate the electricity loss of the cable:
- Estimate service life = 40 years
- Number of conductors = 4 units
- Use rate = 100 percent (according to appendix 1 of the PSR)
- Linear conductor resistivity = 0,00320 Ohm per meter
- Current intensity = 1 Ampere
Module C1 = For both buildings and construction works, cables will be taken out as part of a larger demolition. The energy use for cable removal
compared to other heaver materials is assumed to be low. This module can therefore be included with zero impact.
Module C2 = Estamated average of 85km (Scandinavian standard).
Modules C3 and C4 = Waste treatment of the product follows the default values provided in EN 50693, Product Category Rules for life cycle
assessments of electronic and electrical products and systems, table G.4. This table specified how different types of raw materials used in A1 will
likely be treated during the end-of-life of the product. Waste treatments in C3 include material recycling and incineration with and without energy
recovery and fly ash extraction. Disposal in C4 consist of landfilling of different waste fractions and of ashes.
Module D = The recyclability of metals and plastics allows the producers a credit for the net scrap that is produced at the end of a product’s life.
The benefits from recycling of net scrap are described in formula from EN 15804:2012+A2:2019. Substitution of heat and electricity generated by
the incineration with energy recovery of plastic insulation and other parts is also calculated in module D.
TTrraannssppoorrtt ffrroomm pprroodduuccttiioonn ppllaaccee ttoo uusseerr CCaappaacciittyy uuttiilliissaattiioonn VVaalluuee
DDiissttaannccee ((kkmm)) FFuueell//EEnneerrggyy CCoonnssuummppttiioonn UUnniitt
((AA44)) ((iinnccll.. rreettuurrnn)) %% ((LLiitteerr//ttoonnnnee))
Truck, 16-32 tonnes, EURO 6 (km) 36,7 % 350 0,043 l/tkm 15,05
AAsssseemmbbllyy ((AA55)) UUnniitt VVaalluuee
Product loss during installation (percentage of
Units/DU 0,02
cable)
Waste, packaging, wooden drums, reusable (reuse
cycles:10), 100% recycled, to average treatment kg 0,36
(kg) - A5, incl. 85 km transp.
OOppeerraattiioonnaall eenneerrggyy ((BB66)) UUnniitt VVaalluuee
Electricity, Sweden (kWh) kWh/DU 0,11
CCaappaacciittyy uuttiilliissaattiioonn VVaalluuee
TTrraannssppoorrtt ttoo wwaassttee pprroocceessssiinngg ((CC22)) DDiissttaannccee ((kkmm)) FFuueell//EEnneerrggyy CCoonnssuummppttiioonn UUnniitt
((iinnccll.. rreettuurrnn)) %% ((LLiitteerr//ttoonnnnee))
Truck, 16-32 tonnes, EURO 5 (km) 36,7 % 85 0,044 l/tkm 3,74
WWaassttee pprroocceessssiinngg ((CC33)) UUnniitt VVaalluuee
Aluminium to recycling (kg) kg 0,68
Waste treatment of polyethylene (PE),
incineration with energy recovery and fly ash kg 0,10
extraction (kg)
Copper to recycling (kg) kg 0,15
Waste treatment of plastic mixture, incineration
kg 0,18
with energy recovery and fly ash extraction (kg)
DDiissppoossaall ((CC44)) UUnniitt VVaalluuee
Landfilling of aluminium (kg) kg 0,29
Landfilling of plastic mixture (kg) kg 0,28
Landfilling of ashes from incineration of
Polyethylene (PE), process per kg ashes and kg 0,00
residues (kg)
Landfilling of copper (kg) kg 0,10
Landfilling of ashes from incineration of Plastic
kg 0,01
mixture, process per kg ashes and residues (kg)
5 / 12
BBeenneeffiittss aanndd llooaaddss bbeeyyoonndd tthhee ssyysstteemm UUnniitt VVaalluuee
bboouunnddaarriieess ((DD))
Substitution of primary aluminium with net scrap
kg 0,53
(kg)
Substitution of electricity, in Norway (MJ) MJ 0,48
Substitution of thermal energy, district heating, in
MJ 7,22
Norway (MJ)
Substitution of primary copper with net scrap (kg) kg 0,11
6 / 12
LLCCAA:: RReessuullttss
The LCA results are presented below for the declared unit defined on page 2 of the EPD document.
EEnnvviirroonnmmeennttaall iimmppaacctt
IInnddiiccaattoorr UUnniitt A1 A2 A3 A4 A5 B1 B2 B3
GWP-total kg CO2 -eq 1,67E+01 2,21E-01 3,19E-02 1,23E-01 5,04E-01 0 0 0
GWP-fossil kg CO2 -eq 1,68E+01 2,21E-01 2,96E-02 1,23E-01 9,69E-03 0 0 0
GWP-biogenic kg CO2 -eq -3,15E-01 9,13E-05 6,03E-04 5,09E-05 4,94E-01 0 0 0
GWP-luluc kg CO2 -eq 1,95E-01 7,86E-05 1,67E-03 4,38E-05 2,48E-06 0 0 0
ODP kg CFC11 -eq 1,32E-06 5,00E-08 1,28E-08 2,79E-08 1,55E-09 0 0 0
AP mol H+ -eq 1,63E-01 6,34E-04 1,72E-04 3,53E-04 7,79E-05 0 0 0
EP-FreshWater kg P -eq 1,17E-03 1,76E-06 1,74E-06 9,83E-07 1,16E-07 0 0 0
EP-Marine kg N -eq 1,78E-02 1,26E-04 3,01E-05 6,99E-05 3,34E-05 0 0 0
EP-Terrestial mol N -eq 2,11E-01 1,40E-03 3,91E-04 7,82E-04 3,58E-04 0 0 0
POCP kg NMVOC -eq 6,59E-02 5,38E-04 9,01E-05 3,00E-04 9,20E-05 0 0 0
ADP-minerals&metals1 kg Sb-eq 8,56E-04 6,10E-06 1,05E-06 3,40E-06 1,57E-07 0 0 0
ADP-fossil1 MJ 2,31E+02 3,34E+00 3,02E+00 1,86E+00 1,14E-01 0 0 0
WDP1 m3 6,13E+03 3,23E+00 3,05E+02 1,80E+00 1,75E-01 0 0 0
IInnddiiccaattoorr UUnniitt B4 B5 B6 B7 C1 C2 C3 C4 D
GWP-total kg CO2 -eq 0 0 6,16E-03 0 0 3,05E-02 7,39E-01 3,84E-02 -5,14E+00
GWP-fossil kg CO2 -eq 0 0 5,67E-03 0 0 3,05E-02 7,39E-01 3,83E-02 -5,02E+00
GWP-biogenic kg CO2 -eq 0 0 1,15E-04 0 0 1,24E-05 1,19E-05 3,01E-06 -2,30E-02
GWP-luluc kg CO2 -eq 0 0 3,69E-04 0 0 1,07E-05 2,13E-06 2,86E-06 -9,15E-02
ODP kg CFC11 -eq 0 0 2,78E-09 0 0 6,95E-09 1,18E-09 2,49E-09 -3,05E-03
AP mol H+ -eq 0 0 3,69E-05 0 0 1,25E-04 1,34E-04 6,65E-05 -7,52E-02
EP-FreshWater kg P -eq 0 0 3,84E-07 0 0 2,39E-07 1,07E-07 1,34E-07 -4,76E-04
EP-Marine kg N -eq 0 0 6,29E-06 0 0 3,70E-05 6,40E-05 5,76E-05 -5,91E-03
EP-Terrestial mol N -eq 0 0 8,28E-05 0 0 4,09E-04 6,66E-04 2,67E-04 -7,30E-02
POCP kg NMVOC -eq 0 0 1,89E-05 0 0 1,25E-04 1,60E-04 8,25E-05 -2,27E-02
ADP-minerals&metals1 kg Sb-eq 0 0 2,27E-07 0 0 8,26E-07 5,84E-08 6,55E-08 -2,33E-04
ADP-fossil1 MJ 0 0 6,65E-01 0 0 4,60E-01 7,99E-02 1,97E-01 -6,30E+01
WDP1 m3 0 0 6,75E+01 0 0 4,38E-01 4,79E-01 3,94E+00 -2,70E+03
GWP-total = Global Warming Potential total; GWP-fossil = Global Warming Potential fossil fuels; GWP-biogenic = Global Warming Potential biogenic; GWP-luluc =
Global Warming Potential land use and land use change; ODP = Depletion potential of the stratospheric ozone layer; AP = Acidification potential, Accumulated
Exceedance; EP-freshwater = Eutrophication potential, fraction of nutrients reaching freshwater end compartment: EP-marine = Eutrophication potential, fraction of
nutrients reaching marine end compartment; EP-terrestrial = Eutrophication potential, Accumulated Exceedance; POCP = Formation potential of tropospheric ozone;
ADP-minerals&metals = Abiotic depletion potential for non-fossil resources; ADP-fossil = Abiotic depletion for fossil resources potential; WDP = Water (user)
deprivation potential, deprivation-weighted water consumption
"Reading example: 9,0 E-03 = 9,0*10-3 = 0,009"
*INA Indicator Not Assessed
1. The results of this environmental impact indicator shall be used with care as the uncertainties on these results are high or as there is limited experienced with the
indicator
RReemmaarrkkss ttoo eennvviirroonnmmeennttaall iimmppaaccttss
7 / 12
AAddddiittiioonnaall eennvviirroonnmmeennttaall iimmppaacctt iinnddiiccaattoorrss
IInnddiiccaattoorr UUnniitt A1 A2 A3 A4 A5 B1 B2 B3
PM Disease incidence 1,13E-06 1,35E-08 1,27E-09 7,53E-09 9,52E-10 0 0 0
IRP2 kgBq U235 -eq 8,88E-01 1,46E-02 1,03E-01 8,13E-03 4,13E-04 0 0 0
ETP-fw1 CTUe 1,08E+03 2,47E+00 1,61E+00 1,38E+00 1,30E-01 0 0 0
HTP-c1 CTUh 4,43E-08 0,00E+00 4,60E-11 0,00E+00 1,40E-11 0 0 0
HTP-nc1 CTUh 1,45E-06 2,70E-09 1,12E-09 1,51E-09 6,92E-10 0 0 0
SQP1 dimensionless 4,76E+01 2,33E+00 1,34E+00 1,30E+00 6,38E-02 0 0 0
IInnddiiccaattoorr UUnniitt B4 B5 B6 B7 C1 C2 C3 C4 D
PM Disease incidence 0 0 2,66E-10 0 0 2,19E-09 5,68E-10 1,21E-09 -4,37E-07
IRP2 kgBq U235 -eq 0 0 2,28E-02 0 0 2,01E-03 1,85E-04 1,20E-03 -2,68E-01
ETP-fw1 CTUe 0 0 3,51E-01 0 0 3,39E-01 9,84E-01 2,43E+02 -4,69E+02
HTP-c1 CTUh 0 0 1,00E-11 0 0 0,00E+00 3,20E-11 1,30E-11 -1,76E-08
HTP-nc1 CTUh 0 0 2,43E-10 0 0 3,66E-10 1,41E-09 2,54E-10 -6,20E-07
SQP1 dimensionless 0 0 2,94E-01 0 0 3,17E-01 1,34E-02 4,78E-01 -9,53E+00
PM = Particulate Matter emissions; IRP = Ionizing radiation – human health; ETP-fw = Eco toxicity – freshwater; HTP-c = Human toxicity – cancer effects; HTP-nc =
Human toxicity – non cancer effects; SQP = Potential Soil Quality Index (dimensionless)
"Reading example: 9,0 E-03 = 9,0*10-3 = 0,009"
*INA Indicator Not Assessed
1. The results of this environmental impact indicator shall be used with care as the uncertainties on these results are high or as there is limited experienced with the
indicator
2. This impact category deals mainly with the eventual impact of low dose ionizing radiation on human health of the nuclear fuel cycle. It does not consider effects due
to possible nuclear accidents, occupational exposure nor due to radioactive waste disposal in underground facilities. Potential ionizing radiation from the soil, from
radon and from some construction materials is also not measured by this indicator.
8 / 12
RReessoouurrccee uussee
IInnddiiccaattoorr UUnniitt A1 A2 A3 A4 A5 B1 B2 B3
PERE MJ 5,67E+01 4,78E-02 1,45E+00 2,66E-02 2,34E-03 0 0 0
PERM MJ 4,53E+00 0,00E+00 0,00E+00 0,00E+00 -4,53E+00 0 0 0
PERT MJ 6,13E+01 4,78E-02 1,45E+00 2,66E-02 -4,53E+00 0 0 0
PENRE MJ 2,14E+02 3,34E+00 3,03E+00 1,86E+00 1,14E-01 0 0 0
PENRM MJ 1,73E+01 0,00E+00 0,00E+00 0,00E+00 0,00E+00 0 0 0
PENRT MJ 2,32E+02 3,34E+00 3,03E+00 1,86E+00 1,14E-01 0 0 0
SM kg 5,55E-01 0,00E+00 1,01E-06 0,00E+00 3,60E-01 0 0 0
RSF MJ 4,61E-01 1,71E-03 5,61E-03 9,52E-04 6,82E-05 0 0 0
NRSF MJ 4,61E-02 6,11E-03 1,77E-02 3,41E-03 7,77E-04 0 0 0
FW m3 3,39E-01 3,57E-04 3,29E-03 1,99E-04 8,29E-05 0 0 0
IInnddiiccaattoorr UUnniitt B4 B5 B6 B7 C1 C2 C3 C4 D
PERE MJ 0 0 3,20E-01 0 0 6,49E-03 3,93E-03 2,13E-02 -2,64E+01
PERM MJ 0 0 0,00E+00 0 0 0,00E+00 0,00E+00 0,00E+00 0,00E+00
PERT MJ 0 0 3,20E-01 0 0 6,49E-03 3,93E-03 2,13E-02 -2,64E+01
PENRE MJ 0 0 6,66E-01 0 0 4,60E-01 7,99E-02 1,97E-01 -6,30E+01
PENRM MJ 0 0 0,00E+00 0 0 0,00E+00 -1,70E+01 0,00E+00 0,00E+00
PENRT MJ 0 0 6,66E-01 0 0 4,60E-01 -1,69E+01 1,97E-01 -6,30E+01
SM kg 0 0 0,00E+00 0 0 0,00E+00 0,00E+00 0,00E+00 7,47E-02
RSF MJ 0 0 1,24E-03 0 0 2,32E-04 8,82E-05 4,42E-04 -2,42E-03
NRSF MJ 0 0 3,91E-03 0 0 8,29E-04 0,00E+00 4,83E-04 -1,72E-01
FW m3 0 0 7,26E-04 0 0 4,84E-05 5,64E-04 2,53E-04 -1,30E-01
PERE = Use of renewable primary energy excluding renewable primary energy resources used as raw materials; PERM = Use of renewable primary energy resources used
as raw materials; PERT = Total use of renewable primary energy resources; PENRE = Use of non renewable primary energy excluding non-renewable primary energy
resources used as raw materials; PENRM = Use of non renewable primary energy resources used as raw materials; PENRT = Total use of non renewable primary energy
resources; SM = Use of secondary materials; RSF = Use of renewable secondary fuels; NRSF = Use of non-renewable secondary fuels; FW = Net use of fresh water
"Reading example: 9,0 E-03 = 9,0*10-3 = 0,009"
*INA Indicator Not Assessed
9 / 12
EEnndd ooff lliiffee -- WWaassttee
IInnddiiccaattoorr UUnniitt A1 A2 A3 A4 A5 B1 B2 B3
HWD kg 1,66E-01 1,72E-04 3,42E-04 9,59E-05 0,00E+00 0 0 0
NHWD kg 4,24E+00 1,62E-01 6,91E-02 9,04E-02 3,60E-01 0 0 0
RWD kg 8,35E-04 2,27E-05 4,54E-05 1,27E-05 0,00E+00 0 0 0
IInnddiiccaattoorr UUnniitt B4 B5 B6 B7 C1 C2 C3 C4 D
HWD kg 0 0 3,48E-05 0 0 2,34E-05 0,00E+00 1,78E-02 1,70E-02
NHWD kg 0 0 2,20E-03 0 0 2,20E-02 0,00E+00 6,84E-01 -1,51E+00
RWD kg 0 0 1,00E-05 0 0 3,13E-06 0,00E+00 1,35E-06 -2,51E-04
HWD = Hazardous waste disposed; NHWD = Non-hazardous waste disposed; RWD = Radioactive waste disposed
"Reading example: 9,0 E-03 = 9,0*10-3 = 0,009"
*INA Indicator Not Assessed
EEnndd ooff lliiffee -- OOuuttppuutt ffllooww
IInnddiiccaattoorr UUnniitt A1 A2 A3 A4 A5 B1 B2 B3
CRU kg 0,00E+00 0,00E+00 0,00E+00 0,00E+00 0,00E+00 0 0 0
MFR kg 0,00E+00 0,00E+00 6,28E-02 0,00E+00 8,52E-06 0 0 0
MER kg 0,00E+00 0,00E+00 1,56E-03 0,00E+00 3,60E-01 0 0 0
EEE MJ 0,00E+00 0,00E+00 2,12E-03 0,00E+00 2,50E-01 0 0 0
EET MJ 0,00E+00 0,00E+00 3,20E-02 0,00E+00 3,79E+00 0 0 0
IInnddiiccaattoorr UUnniitt B4 B5 B6 B7 C1 C2 C3 C4 D
CRU kg 0 0 0,00E+00 0 0 0,00E+00 0,00E+00 0,00E+00 0,00E+00
MFR kg 0 0 0,00E+00 0 0 0,00E+00 8,30E-01 2,55E-05 -2,93E-03
MER kg 0 0 0,00E+00 0 0 0,00E+00 2,85E-01 6,24E-07 -3,85E-04
EEE MJ 0 0 0,00E+00 0 0 0,00E+00 4,78E-01 4,05E-05 -9,44E-04
EET MJ 0 0 0,00E+00 0 0 0,00E+00 7,22E+00 6,13E-04 -1,43E-02
CRU = Components for re-use; MFR = Materials for recycling; MER = Materials for energy recovery; EEE = Exported energy electrical; EET = Exported energy thermal
"Reading example: 9,0 E-03 = 9,0*10-3 = 0,009"
*INA Indicator Not Assessed
BBiiooggeenniicc CCaarrbboonn CCoonntteenntt
IInnddiiccaattoorr UUnniitt AAtt tthhee ffaaccttoorryy ggaattee
Biogenic carbon content in product kg C 0,00E+00
Biogenic carbon content in accompanying packaging kg C 1,35E-01
Note: 1 kg biogenic carbon is equivalent to 44/12 kg CO2
10 / 12
AAddddiittiioonnaall rreeqquuiirreemmeennttss
GGrreeeennhhoouussee ggaass eemmiissssiioonnss ffrroomm tthhee uussee ooff eelleeccttrriicciittyy iinn tthhee mmaannuuffaaccttuurriinngg pphhaassee
National production mix from import, low voltage (production of transmission lines, in addition to direct emissions and losses in grid) of applied
electricity for the manufacturing process (A3).
EElleeccttrriicciittyy mmiixx SSoouurrccee AAmmoouunntt UUnniitt
Electricity, Sweden (kWh) ecoinvent 3.6 54,94 g CO2-eq/kWh
DDaannggeerroouuss ssuubbssttaanncceess
The product contains no substances given by the REACH Candidate list.
IInnddoooorr eennvviirroonnmmeenntt
AAddddiittiioonnaall EEnnvviirroonnmmeennttaall IInnffoorrmmaattiioonn
AAddddiittiioonnaall eennvviirroonnmmeennttaall iimmppaacctt iinnddiiccaattoorrss rreeqquuiirreedd iinn NNPPCCRR PPaarrtt AA ffoorr ccoonnssttrruuccttiioonn pprroodduuccttss
IInnddiiccaattoorr UUnniitt A1 A2 A3 A4 A5 B1 B2 B3
GWPIOBC kg CO2 -eq 1,71E+01 2,21E-01 3,18E-02 1,23E-01 9,69E-03 0 0 0
IInnddiiccaattoorr UUnniitt B4 B5 B6 B7 C1 C2 C3 C4 D
GWPIOBC kg CO2 -eq 0 0 6,15E-03 0 0 3,05E-02 7,39E-01 4,00E-02 -4,78E+00
GWP-IOBC: Global warming potential calculated according to the principle of instantaneous oxidation. In order to increase the transparency of biogenic carbon​
contribution to climate impact, the indicator GWP-IOBC is required as it declares climate impacts calculated according to the principle of instantaneous oxidation.​
GWP-IOBC is also referred to as GWP-GHG in context to Swedish public procurement legislation.
11 / 12
BBiibblliiooggrraapphhyy
ISO 14025:2010. Environmental labels and declarations - Type III environmental declarations - Principles and procedures. International
Organization for Standardization.
ISO 14044:2006. Environmental management - Life cycle assessment - Requirements and guidelines. International Organization for
Standardization.
EN 15804:2012+A2:2019. Environmental product declaration - Core rules for the product category of construction products. European
Committee for Standardization.
ISO 21930:2017. Sustainability in buildings and civil engineering works - Core rules for environmental product declarations of construction
products. International Organization for Standardization.
EN 50693:2019. Product category rules for life cycle assessments of electronic and electrical products and systems. European Committee for
Standardization.
Ecoinvent v3, 2019. Allocation, cut-off by classification. Swiss Centre of Life Cycle Inventories.
Iversen et al., (2021). eEPD v2021.09, background information for EPD generator tool system verification, LCA.no. Report number: 07.21. System
verification report.
Philis et al., (2022). EPD generator for NPCR 027 part B for electrical wires and cables, background information for EPD generator application and
LCA data, LCA.no Report number: 03.22. PCR verification report.
EPD Norway (2022). NPCR Part A: Construction products and services. The Norwegian EPD foundation. Version 2.0 published 24.03.2021.
EPD Norway (2022). NPCR 027 Part B for electrical cables and wires. The Norwegian EPD foundation. Version 2.0 published 01.03.2022.
PPrrooggrraamm ooppeerraattoorr aanndd ppuubblliisshheerr Phone: +47 977 22 020
The Norwegian EPD Foundation e-mail: post@epd-norge.no
Post Box 5250 Majorstuen, 0303 Oslo, Norway web: www.epd-norge.no
OOwwnneerr ooff tthhee ddeeccllaarraattiioonn:: Phone: +46 481-750 810
Amokabel AB e-mail: oskar.wijk@amokabel.com
Kabelvägen 5, SE-36443 Alstermo, Sweden web: www.amokabel.com
AAuutthhoorr ooff tthhee LLiiffee CCyyccllee AAsssseessssmmeenntt Phone: +47 916 50 916
LCA.no AS e-mail: post@lca.no
Dokka 6A, 1671 Kråkerøy, Norway web: www.lca.no
DDeevveellooppeerr ooff EEPPDD ggeenneerraattoorr Phone: +47 916 50 916
LCA.no AS e-mail: post@lca.no
Dokka 6A, 1671 Kråkerøy, Norway web: www.lca.no
ECO Platform web: www.eco-platform.org
ECO Portal web: ECO Portal
12 / 12
