Environmental product declaration
in accordance with ISO 14025 and EN 15804+A2
Tec-Flex 5 G10 +2 X1,5 0,6/1,0kV RV-K
Owner of the declaration: Program operator:
Onninen AS The Norwegian EPD
Foundation
Product:
Tec-Flex 5 G10 +2 X1,5 0,6/1,0kV RV-K Declaration number:
NEPD-8091-7762-EN
Declared unit:
1 m Registration number:
NEPD-8091-7762-EN
This declaration is based on Product
Category Rules: Issue date:
CEN Standard EN 15804:2012+A2:2019 14.11.2024
serves as core PCR
Valid to:
NPCR 027:2020 Part B for Electrical cables and
14.11.2029
The Norwegian EPD Foundation wires
EPD software:
LCAno EPD generator ID:
600899
1 / 12
General information
Product Owner of the declaration:
Tec-Flex 5 G10 +2 X1,5 0,6/1,0kV RV-K Onninen AS
Contact person: Nils - Arne Grande
Phone: +47 97 66 22 12
e-mail: nils-arne.grande@onninen.com
Program operator: Manufacturer:
The Norwegian EPD Foundation TECCON Norge AS
Post Box 5250 Majorstuen, 0303 Oslo, Norway Mekjarvik 18
Phone: +47 977 22 020 4072 Randaberg, Norway
web: www.epd-norge.no
Declaration number: Place of production:
Teccon production site Léon (Spain
NEPD-8091-7762-EN
, Spain
This declaration is based on Product Category Rules: Management system:
CEN Standard EN 15804:2012+A2:2019 serves as core PCR ISO 14001, ISO 9001
NPCR 027:2020 Part B for Electrical cables and wires
Statement of liability: Organisation no:
The owner of the declaration shall be liable for the underlying 979 692 900
information and evidence. EPD Norway shall not be liable with respect
to manufacturer information, life cycle assessment data and
evidences.​
Declared unit: Issue date:
1 m Tec-Flex 5 G10 +2 X1,5 0,6/1,0kV RV-K 14.11.2024
Declared unit with option: Valid to:
A1,A2,A3,A4,A5,B6,C1,C2,C3,C4,D 14.11.2029
Year of study:
2023
Functional unit: Comparability:
EPD of construction products may not be comparable if they not
comply with EN 15804 and seen in a building context.
General information on verification of EPD from EPD tools: Development and verification of EPD:
Independent verification of data, other environmental information The declaration is created using EPD tool lca.tools ver EPD2022.03,
and the declaration according to ISO 14025:2010, § 8.1.3 and § 8.1.4. developed by LCA.no. The EPD tool is integrated in the company's
Verification of each EPD is made according to EPD-Norway’s management system, and has been approved by EPD Norway.
guidelines for verification and approval requiring that tools are i) Approval number:
integrated into the company's environmental management system, ii)
the procedures for use of the EPD tool are approved by EPD-Norway, Developer of EPD: Jan Vestergaard, Teccon Norge AS
and iii) the process is reviewed annually by an independent third
Reviewer of company-specific input data and EPD:​ Nils Arne Grande,
party verifier. See Appendix G of EPD-Norway's General Programme
Onninen AS
Instructions for further information on EPD tools
Verification of EPD tool: Approved:
Independent third party verification of the EPD tool, background data
and test-EPD in accordance with EPDNorway's procedures and
guidelines for verification and approval of EPD tools. Approval
number: NEPDT32.
Håkon Hauan, CEO EPD-Norge
Third party verifier:
Vito D’Incognito, Take Care International
(no signature required)
2 / 12
Product
Product description:
Tec Flex RV-K 0,6/1 kV power cables are specially indicated for its use in distribution networks, power stations, industries or buildings, and electrical
installations in steel ships.
For electrical energy transport and distribution, distribution networks, protected or not. For indoor and outdoor installations. Non-suitable for
facilities of feeding of submerged pumps
Surface mounted (directly installed or on cable trays, cable ladders, cleats, brackets or in cable ducting (conduit, pipes or similar closed systems)).
Embedded (directly or in cable ducting).
In building voids and cavities (directly or on cable trays, cable ladders, in cable ducting).
Buried in ground (directly or in conduit)
Texflex combi are with two commonication conductors for service off CMS.
Product specification
General: UNE 21-123-91; IEC 60502-21-123-91/1; HD 603-1​
Flexible installation cable 0,6/1,0kV
Materials kg %
Copper conductor 0,41 48,75
Plastic - Polyethylene 0,05 6,45
Plastic - Polyvinyl chloride (PVC) 0,15 17,92
Total 0,61 73,12
Packaging kg %
Packaging - Wood 0,23 26,88
Total incl. packaging 0,84 26,88
Technical data:
Cable​
Standard IEC 60502-1​
Conductor Annealed electrolytic flexible multi-stranded copper conductor, class 5, IEC 60228​
Insulation XLPE – according to standard IEC 60502-1​
Coloured According to HD 308 S2​
Colour code Cenelec. Yellow/Green; Blue, brown, Black, Grey​
Bedding PVC​
Jacket PVC, White or Grey. UV stabilized. (PVC type ST2 according to IEC 60502-1)​
Marking RV-K 0,6/1,0kV xx G mm² Year/lot​
Rated Voltage U0/U 0,6/1,0kV​
Volatge test 3500V​
Service temp 90° C​
Short circuit temp 250° C​
Fire performance EN 50575:2014+A1:2016​
Flame retardant EN 60332-1-2​
CPR EN50575 Eca​
Temperature – service -25- 60°​
Temperature – installation 0 - 50°​
Bending radius 10 x D​
Marking – Approvals – directives​
RohS​
Low Voltage Directive​
CPR compliant​
Marine approval​
Registered for use in Swan Buildings​
Market:
Nordic
Reference service life, product
30Y+
Reference service life, building or construction works
30Y+
3 / 12
LCA: Calculation rules
Declared unit:
1 m Tec-Flex 5 G10 +2 X1,5 0,6/1,0kV RV-K
Cut-off criteria:
All major raw materials and all the essential energy is included. The production processes for raw materials and energy flows with very small
amounts (less than 1%) are not included. These cut-off criteria do not apply for hazardous materials and substances.
All major materials have been included. Substance representing <1% have not been included. This include folio film for packaging!
Allocation:
The allocation is made in accordance with the provisions of EN 15804. Incoming energy and water and waste production in-house is allocated
equally among all products through mass allocation. Effects of primary production of recycled materials is allocated to the main product in which
the material was used. The recycling process and transportation of the material is allocated to this analysis. The allocation is made in accordance
with the guidelines given in EN 15804.​
Raw material - Information derived from manufactory and from a LCA generator​
Processing: Derived from actual measurements during production of the individual units/stages​
Data quality:
Specific data for the product composition are provided by the manufacturer. The data represent the production of the declared product and were
collected for EPD development in the year of study. Background data is based on EPDs according to EN 15804 and different LCA databases. The
data quality of the raw materials in A1 is presented in the table below.
Data from material supplier and the LCA generator has been accepted "As-Is"​
Data from processing TECCON in-house has been repeated ongoingly without major deviations. Figures given in document are worst case values.​
Materials Source Data quality Year
Copper conductor ecoinvent 3.6 Database 2019
Packaging - Wood Modified ecoinvent 3.6 Database 2019
Plastic - Polyethylene ecoinvent 3.6 Database 2019
Plastic - Polyvinyl chloride (PVC) ecoinvent 3.6 Database 2019
4 / 12
System boundaries (X=included, MND=module not declared, MNR=module not relevant)
Construction Beyond the system
Product stage Use stage End of life stage
installation stage boundaries
A1 A2 A3 A4 A5 B1 B2 B3 B4 B5 B6 B7 C1 C2 C3 C4 D
X X X X X MND MND MND MND MND X MND X X X X X
System boundary:
Cradle to Gate.​
The following stages have been declared: A1-A4​
The flowchart below illustrates the system boundaries of the analysis:
Additional technical information:
Article 1010462 Tec-Flex combi. 5G 10 + 2,5 0,6/1,0kV RV-K cable represent the maximum energy consumption from the product family below -
from a production volume perspective as follow:
1010460 7042720002134 Tec-Flex 4G10mm² + 2x1,5mm²
1010461 7042720002141 Tec-Flex 4G16mm² + 2x1,5mm²
1010462 7042720002158 Tec-Flex 5G10mm² + 2x1,5mm²
1010463 7042720002165 Tec-Flex 5G16mm² + 2x1,5mm²
If required individual EPD may be conducted accordingly!
waR slairetam tropsnarT gnirutcafunaM tropsnarT ylbmessA e​sU ecnanetniaM riapeR tnemecalpeR tnemhsibrufeR lanoitarepO ygrene esu lanoitarepO esu retaw -eD noitcurtsnoc noitilomed tropsnarT etsaW gnissecorp lasopsiD -yrevoceR-esueR laitnetop-gnilcyceR
5 / 12
LCA: Scenarios and additional technical information
The following information describe the scenarios in the different modules of the EPD.
Capacity utilisation Value
Transport from production place to user (A4) Distance (km) Fuel/Energy Consumption Unit
(incl. return) % (Liter/tonne)
Truck, 16-32 tonnes, EURO 6 (km) 36,7 % 988 0,043 l/tkm 42,48
Assembly (A5) Unit Value
Waste, wood, to average treatment - A5 including
kg 0,23
transport (kg)
Operational energy (B6) Unit Value
Electricity, Norway (kWh) kWh/DU 0,01
Capacity utilisation Value
Transport to waste processing (C2) Distance (km) Fuel/Energy Consumption Unit
(incl. return) % (Liter/tonne)
Truck, 16-32 tonnes, EURO 6 (km) 36,7 % 300 0,043 l/tkm 12,90
Waste processing (C3) Unit Value
Waste treatment of polyethylene (PE),
incineration with energy recovery and fly ash kg 0,03
extraction (kg)
Waste treatment of plastic mixture, incineration
kg 0,08
with energy recovery and fly ash extraction (kg)
Copper to recycling (kg) kg 0,24
Disposal (C4) Unit Value
Landfilling of plastic mixture (kg) kg 0,10
Landfilling of ashes from incineration of
Polyethylene (PE), process per kg ashes and kg 0,00
residues (kg)
Landfilling of copper (kg) kg 0,16
Landfilling of ashes from incineration of Plastic
kg 0,00
mixture, process per kg ashes and residues (kg)
Benefits and loads beyond the system
Unit Value
boundaries (D)
Substitution of primary copper with net scrap (kg) kg 0,17
Substitution of electricity, in Norway (MJ) MJ 0,17
Substitution of thermal energy, district heating, in
MJ 2,54
Norway (MJ)
6 / 12
LCA: Results
The LCA results are presented below for the declared unit defined on page 2 of the EPD document.
Environmental impact
Indicator Unit A1 A2 A3 A4 A5
GWP-total kg CO2 -eq 2,40E+00 9,36E-02 1,03E-01 1,35E-01 3,47E-01
GWP-fossil kg CO2 -eq 2,69E+00 9,35E-02 1,01E-01 1,35E-01 6,05E-03
GWP-biogenic kg CO2 -eq -2,94E-01 3,63E-05 2,92E-04 5,59E-05 3,41E-01
GWP-luluc kg CO2 -eq 2,66E-03 3,91E-05 9,06E-04 4,81E-05 1,55E-06
ODP kg CFC11 -eq 3,11E-07 2,09E-08 1,11E-08 3,06E-08 9,67E-10
AP mol H+ -eq 1,07E-01 7,81E-04 9,13E-04 3,88E-04 4,87E-05
EP-FreshWater kg P -eq 8,76E-04 6,81E-07 4,84E-06 1,08E-06 7,26E-08
EP-Marine kg N -eq 7,14E-03 1,81E-04 1,30E-04 7,68E-05 2,09E-05
EP-Terrestial mol N -eq 1,04E-01 2,02E-03 1,47E-03 8,59E-04 2,24E-04
POCP kg NMVOC -eq 2,70E-02 5,84E-04 3,94E-04 3,29E-04 5,75E-05
ADP-minerals&metals1 kg Sb-eq 5,06E-03 2,23E-06 8,30E-07 3,73E-06 9,82E-08
ADP-fossil1 MJ 4,23E+01 1,37E+00 2,35E+00 2,04E+00 7,11E-02
WDP1 m3 2,00E+02 1,16E+00 -5,35E+01 1,98E+00 1,10E-01
Indicator Unit B6 C1 C2 C3 C4 D
GWP-total kg CO2 -eq 2,94E-04 0 4,10E-02 2,59E-01 1,41E-02 -4,19E-01
GWP-fossil kg CO2 -eq 2,85E-04 0 4,10E-02 2,59E-01 1,41E-02 -4,16E-01
GWP-biogenic kg CO2 -eq 7,89E-06 0 1,70E-05 4,52E-06 1,07E-06 -1,90E-03
GWP-luluc kg CO2 -eq 1,18E-06 0 1,46E-05 8,16E-07 1,15E-06 -9,30E-04
ODP kg CFC11 -eq 2,00E-11 0 9,29E-09 4,48E-10 9,79E-10 -1,07E-03
AP mol H+ -eq 2,23E-06 0 1,18E-04 4,91E-05 2,63E-05 -6,75E-02
EP-FreshWater kg P -eq 2,05E-08 0 3,28E-07 4,05E-08 5,38E-08 -4,55E-04
EP-Marine kg N -eq 2,45E-07 0 2,33E-05 2,35E-05 2,15E-05 -2,81E-03
EP-Terrestial mol N -eq 3,19E-06 0 2,61E-04 2,44E-04 1,06E-04 -4,33E-02
POCP kg NMVOC -eq 8,58E-07 0 9,99E-05 5,87E-05 3,24E-05 -1,18E-02
ADP-minerals&metals1 kg Sb-eq 2,13E-08 0 1,13E-06 2,23E-08 2,59E-08 -3,78E-04
ADP-fossil1 MJ 3,89E-03 0 6,20E-01 2,97E-02 7,80E-02 -3,79E+00
WDP1 m3 6,79E-01 0 6,00E-01 1,88E-01 1,60E+00 1,93E+01
GWP-total = Global Warming Potential total; GWP-fossil = Global Warming Potential fossil fuels; GWP-biogenic = Global Warming Potential biogenic; GWP-luluc =
Global Warming Potential land use and land use change; ODP = Depletion potential of the stratospheric ozone layer; AP = Acidification potential, Accumulated
Exceedance; EP-freshwater = Eutrophication potential, fraction of nutrients reaching freshwater end compartment: EP-marine = Eutrophication potential, fraction of
nutrients reaching marine end compartment; EP-terrestrial = Eutrophication potential, Accumulated Exceedance; POCP = Formation potential of tropospheric ozone;
ADP-minerals&metals = Abiotic depletion potential for non-fossil resources; ADP-fossil = Abiotic depletion for fossil resources potential; WDP = Water (user)
deprivation potential, deprivation-weighted water consumption
"Reading example: 9,0 E-03 = 9,0*10-3 = 0,009"
*INA Indicator Not Assessed
1. The results of this environmental impact indicator shall be used with care as the uncertainties on these results are high or as there is limited experienced with the
indicator
Remarks to environmental impacts
7 / 12
Additional environmental impact indicators
Indicator Unit A1 A2 A3 A4 A5
PM Disease incidence 3,12E-07 4,67E-09 2,11E-09 8,27E-09 5,95E-10
IRP2 kgBq U235 -eq 1,72E-01 5,99E-03 2,54E-02 8,93E-03 2,58E-04
ETP-fw1 CTUe 1,26E+03 9,83E-01 1,95E+00 1,51E+00 8,10E-02
HTP-c1 CTUh 2,19E-08 0,00E+00 5,00E-11 0,00E+00 9,00E-12
HTP-nc1 CTUh 1,67E-06 9,34E-10 1,71E-09 1,65E-09 4,32E-10
SQP1 dimensionless 3,33E+01 8,36E-01 5,06E-01 1,43E+00 3,99E-02
Indicator Unit B6 C1 C2 C3 C4 D
PM Disease incidence 1,60E-11 0 2,51E-09 2,10E-10 4,75E-10 -1,42E-07
IRP2 kgBq U235 -eq 7,07E-05 0 2,71E-03 7,04E-05 4,78E-04 -5,80E-03
ETP-fw1 CTUe 1,77E-02 0 4,60E-01 3,91E-01 1,01E+02 -6,21E+02
HTP-c1 CTUh 1,00E-12 0 0,00E+00 1,20E-11 5,00E-12 -8,77E-09
HTP-nc1 CTUh 2,00E-11 0 5,02E-10 5,36E-10 1,01E-10 -7,51E-07
SQP1 dimensionless 1,96E-03 0 4,34E-01 5,10E-03 1,84E-01 -9,27E+00
PM = Particulate Matter emissions; IRP = Ionizing radiation – human health; ETP-fw = Eco toxicity – freshwater; HTP-c = Human toxicity – cancer effects; HTP-nc =
Human toxicity – non cancer effects; SQP = Potential Soil Quality Index (dimensionless)
"Reading example: 9,0 E-03 = 9,0*10-3 = 0,009"
*INA Indicator Not Assessed
1. The results of this environmental impact indicator shall be used with care as the uncertainties on these results are high or as there is limited experienced with the
indicator
2. This impact category deals mainly with the eventual impact of low dose ionizing radiation on human health of the nuclear fuel cycle. It does not consider effects due
to possible nuclear accidents, occupational exposure nor due to radioactive waste disposal in underground facilities. Potential ionizing radiation from the soil, from
radon and from some construction materials is also not measured by this indicator.
8 / 12
Resource use
Indicator Unit A1 A2 A3 A4 A5
PERE MJ 8,21E+00 1,80E-02 6,18E-01 2,92E-02 1,46E-03
PERM MJ 3,12E+00 0,00E+00 0,00E+00 0,00E+00 -3,12E+00
PERT MJ 1,13E+01 1,80E-02 6,18E-01 2,92E-02 -3,12E+00
PENRE MJ 3,71E+01 1,37E+00 2,35E+00 2,04E+00 7,12E-02
PENRM MJ 5,43E+00 0,00E+00 0,00E+00 0,00E+00 0,00E+00
PENRT MJ 4,25E+01 1,37E+00 2,35E+00 2,04E+00 7,12E-02
SM kg 7,69E-02 0,00E+00 0,00E+00 0,00E+00 0,00E+00
RSF MJ 2,18E-01 6,27E-04 4,09E-03 1,05E-03 4,26E-05
NRSF MJ 6,58E-03 2,62E-03 1,10E-02 3,74E-03 4,86E-04
FW m3 4,58E-02 1,35E-04 1,04E-03 2,18E-04 5,18E-05
Indicator Unit B6 C1 C2 C3 C4 D
PERE MJ 5,04E-02 0 8,88E-03 1,52E-03 8,67E-03 -2,74E+00
PERM MJ 0,00E+00 0 0,00E+00 0,00E+00 0,00E+00 0,00E+00
PERT MJ 5,04E-02 0 8,88E-03 1,52E-03 8,67E-03 -2,74E+00
PENRE MJ 3,90E-03 0 6,20E-01 2,97E-02 7,80E-02 -3,79E+00
PENRM MJ 0,00E+00 0 0,00E+00 -5,43E+00 0,00E+00 0,00E+00
PENRT MJ 3,90E-03 0 6,20E-01 -5,40E+00 7,80E-02 -3,79E+00
SM kg 0,00E+00 0 0,00E+00 0,00E+00 0,00E+00 1,17E-01
RSF MJ 3,96E-05 0 3,18E-04 3,36E-05 1,80E-04 1,09E-02
NRSF MJ 9,87E-05 0 1,14E-03 0,00E+00 1,43E-04 -5,29E-02
FW m3 3,77E-04 0 6,63E-05 2,21E-04 1,01E-04 -1,14E-02
PERE = Use of renewable primary energy excluding renewable primary energy resources used as raw materials; PERM = Use of renewable primary energy resources used
as raw materials; PERT = Total use of renewable primary energy resources; PENRE = Use of non renewable primary energy excluding non-renewable primary energy
resources used as raw materials; PENRM = Use of non renewable primary energy resources used as raw materials; PENRT = Total use of non renewable primary energy
resources; SM = Use of secondary materials; RSF = Use of renewable secondary fuels; NRSF = Use of non-renewable secondary fuels; FW = Net use of fresh water
"Reading example: 9,0 E-03 = 9,0*10-3 = 0,009"
*INA Indicator Not Assessed
9 / 12
End of life - Waste
Indicator Unit A1 A2 A3 A4 A5
HWD kg 3,16E-02 6,89E-05 1,31E-04 1,05E-04 0,00E+00
NHWD kg 8,98E-01 5,66E-02 9,31E-03 9,93E-02 2,25E-01
RWD kg 1,63E-04 9,39E-06 1,81E-05 1,39E-05 0,00E+00
Indicator Unit B6 C1 C2 C3 C4 D
HWD kg 2,50E-06 0 3,20E-05 0,00E+00 6,99E-03 -4,56E-03
NHWD kg 3,00E-04 0 3,02E-02 0,00E+00 2,68E-01 -1,98E-01
RWD kg 3,49E-08 0 4,22E-06 0,00E+00 5,35E-07 -5,13E-06
HWD = Hazardous waste disposed; NHWD = Non-hazardous waste disposed; RWD = Radioactive waste disposed
"Reading example: 9,0 E-03 = 9,0*10-3 = 0,009"
*INA Indicator Not Assessed
End of life - Output flow
Indicator Unit A1 A2 A3 A4 A5
CRU kg 0,00E+00 0,00E+00 0,00E+00 0,00E+00 0,00E+00
MFR kg 0,00E+00 0,00E+00 0,00E+00 0,00E+00 5,32E-06
MER kg 0,00E+00 0,00E+00 0,00E+00 0,00E+00 2,25E-01
EEE MJ 0,00E+00 0,00E+00 0,00E+00 0,00E+00 1,56E-01
EET MJ 0,00E+00 0,00E+00 0,00E+00 0,00E+00 2,37E+00
Indicator Unit B6 C1 C2 C3 C4 D
CRU kg 0,00E+00 0 0,00E+00 0,00E+00 0,00E+00 0,00E+00
MFR kg 0,00E+00 0 0,00E+00 2,45E-01 9,15E-06 -4,59E-03
MER kg 0,00E+00 0 0,00E+00 1,02E-01 2,24E-07 -6,05E-04
EEE MJ 0,00E+00 0 0,00E+00 1,68E-01 1,45E-05 -1,48E-03
EET MJ 0,00E+00 0 0,00E+00 2,54E+00 2,20E-04 -2,24E-02
CRU = Components for re-use; MFR = Materials for recycling; MER = Materials for energy recovery; EEE = Exported energy electrical; EET = Exported energy thermal
"Reading example: 9,0 E-03 = 9,0*10-3 = 0,009"
*INA Indicator Not Assessed
Biogenic Carbon Content
Indicator Unit At the factory gate
Biogenic carbon content in product kg C 0,00E+00
Biogenic carbon content in accompanying packaging kg C 9,30E-02
Note: 1 kg biogenic carbon is equivalent to 44/12 kg CO2
10 / 12
Additional requirements
Greenhouse gas emissions from the use of electricity in the manufacturing phase
National production mix from import, low voltage (production of transmission lines, in addition to direct emissions and losses in grid) of applied
electricity for the manufacturing process (A3).
Electricity mix Source Amount Unit
Electricity, Spain (kWh) ecoinvent 3.6 337,33 g CO2-eq/kWh
Dangerous substances
The product contains no substances given by the REACH Candidate list.
Indoor environment
No effect on in-door environment
Additional Environmental Information
Additional environmental impact indicators required in NPCR Part A for construction products
Indicator Unit A1 A2 A3 A4 A5
GWPIOBC kg CO2 -eq 2,73E+00 9,36E-02 1,06E-01 1,35E-01 6,06E-03
Indicator Unit B6 C1 C2 C3 C4 D
GWPIOBC kg CO2 -eq 2,94E-04 0 4,10E-02 2,59E-01 1,47E-02 -2,05E-01
GWP-IOBC: Global warming potential calculated according to the principle of instantaneous oxidation. In order to increase the transparency of biogenic carbon​
contribution to climate impact, the indicator GWP-IOBC is required as it declares climate impacts calculated according to the principle of instantaneous oxidation.​
GWP-IOBC is also referred to as GWP-GHG in context to Swedish public procurement legislation.
11 / 12
Bibliography
ISO 14025:2010. Environmental labels and declarations - Type III environmental declarations - Principles and procedures. International
Organization for Standardization.
ISO 14044:2006. Environmental management - Life cycle assessment - Requirements and guidelines. International Organization for
Standardization.
EN 15804:2012+A2:2019. Environmental product declaration - Core rules for the product category of construction products. European
Committee for Standardization.
ISO 21930:2017. Sustainability in buildings and civil engineering works - Core rules for environmental product declarations of construction
products. International Organization for Standardization.
EN 50693:2019. Product category rules for life cycle assessments of electronic and electrical products and systems. European Committee for
Standardization.
Ecoinvent v3, 2019. Allocation, cut-off by classification. Swiss Centre of Life Cycle Inventories.
Iversen et al., (2021). eEPD v2021.09, background information for EPD generator tool system verification, LCA.no. Report number: 07.21. System
verification report.
Philis et al., (2022). EPD generator for NPCR 027 part B for electrical wires and cables, background information for EPD generator application and
LCA data, LCA.no Report number: 03.22. PCR verification report.
EPD Norway (2022). NPCR Part A: Construction products and services. The Norwegian EPD foundation. Version 2.0 published 24.03.2021.
EPD Norway (2022). NPCR 027 Part B for electrical cables and wires. The Norwegian EPD foundation. Version 2.0 published 01.03.2022.
Program operator and publisher Phone: +47 977 22 020
The Norwegian EPD Foundation e-mail: post@epd-norge.no
Post Box 5250 Majorstuen, 0303 Oslo, Norway web: www.epd-norge.no
Owner of the declaration: Phone: +47 97 66 22 12
nils-
Onninen AS e-mail:
arne.grande@onninen.com
Postboks 143, 1403 Langhus web: onninen.no
Author of the Life Cycle Assessment Phone: +47 916 50 916
LCA.no AS e-mail: post@lca.no
Dokka 6A, 1671 Kråkerøy web: www.lca.no
Developer of EPD generator Phone: +47 916 50 916
LCA.no AS e-mail: post@lca.no
Dokka 6A, 1671 Kråkerøy web: www.lca.no
ECO Platform web: www.eco-platform.org
ECO Portal web: ECO Portal
12 / 12
