Environmental product declaration
in accordance with ISO 14025 and EN 15804+A2
Lake 01 stackable chair with armrest, upholstered, bolt base
Owner of the declaration: Program operator:
Helland Møbler AS The Norwegian EPD Foundation
Product: Declaration number:
Lake 01 stackable chair with armrest, upholstered, bolt
base NEPD-8537-8202-EN
Declared unit: Registration number:
1 pcs
NEPD-8537-8202-EN
This declaration is based on Product Category Rules:
Issue date: 18.12.2024
CEN Standard EN 15804:2012+A2:2019 serves as core
The Norwegian EPD Foundation PCR Valid to: 18.12.2029
NPCR 026:2022 Part B for Furniture
EPD software:
LCAno EPD generator ID: 712065
1 / 12
General information
Product Owner of the declaration:
Lake 01 stackable chair with armrest, upholstered, bolt base Helland Møbler AS
Contact person: Joakim Helland
Phone: +47 958 09 013
e-mail: joakim.helland@helland.no
Program operator: Manufacturer:
The Norwegian EPD Foundation Helland Møbler AS
Post Box 5250 Majorstuen, 0303 Oslo, Norway Postboks 10
Phone: +47 977 22 020 6259 Stordal, Norway
web: www.epd-norge.no
Declaration number: Place of production:
Helland Baltic ÖU
NEPD-8537-8202-EN
Hapvali, Nõmme küla, Haapsalu linn
EE-90439 Läänemaa, Estonia
This declaration is based on Product Category Rules: Management system:
CEN Standard EN 15804:2012+A2:2019 serves as core PCR ISO 14001:2015, sertifikat nr 901085
NPCR 026:2022 Part B for Furniture
Statement of liability: Organisation no:
The owner of the declaration shall be liable for the underlying 943 511 128
information and evidence. EPD Norway shall not be liable with respect
to manufacturer information, life cycle assessment data and
evidences.​
Declared unit: Issue date:
1 pcs Lake 01 stackable chair with armrest, upholstered, bolt base 18.12.2024
Declared unit (cradle to gate) with option: Valid to:
A1-A3,A4,A5,B2,B3,B4,C1,C2,C3,C4 18.12.2029
Year of study:
2023
Functional unit: Comparability:
Production of one chair provided and maintained for 15 years. EPD of construction products may not be comparable if they not
comply with EN 15804 and seen in a building context.
General information on verification of EPD from EPD tools: Development and verification of EPD:
Independent verification of data, other environmental information The declaration is created using EPD tool lca.tools ver EPD2022.03,
and the declaration according to ISO 14025:2010, § 8.1.3 and § 8.1.4. developed by LCA.no. The EPD tool is integrated in the company's
Verification of each EPD is made according to EPD-Norway’s management system, and has been approved by EPD Norway.
guidelines for verification and approval requiring that tools are i)
integrated into the company's environmental management system, ii) Developer of EPD: Uve Uustalu
the procedures for use of the EPD tool are approved by EPD-Norway,
Reviewer of company-specific input data and EPD: Pawel Sosinski
and iii) the process is reviewed annually by an independent third
party verifier. See Appendix G of EPD-Norway's General Programme
Instructions for further information on EPD tools
Verification of EPD tool: Approved:
Independent third party verification of the EPD tool, background data
and test-EPD in accordance with EPDNorway's procedures and
guidelines for verification and approval of EPD tools.
Third party verifier:
Elisabet Amat, GREENIZE projects
(no signature required)
2 / 12
Product
Product description:
Lake is a minimalist and modern chair, which with its toned-down design language fits in most interiors. The steel base is excellent, stands firmly
on the ground, and comes with the possibility of connection. The chair is soft, and comfortable and has some swaying motion in the back, for a
flexible and relaxed sitting position.
Product specification
• Upholstered back
• Upolstered seat
• With/without armrest
• Bolt base
• Stackable
• Can hang on edge of table
• Chemical disinfectant ok (acid-cured varnish)
• EPD (Environmental Product Declaration)
• Møbelfakta
Recycled share in Recycled share in
Materials kg %
material (kg) material (%)
Plastic - Nylon (PA) 0,12 1,54 0,00 0,00
Plastic -
0,80 10,57 0,00 0,00
Polyurethane (PUR)
Textile - Wool 0,70 9,28 0,00 0,00
Metal - Steel 4,43 58,72 0,89 20,00
Wood - Plywood 1,50 19,89 0,00 0,00
Total 7,54 100,00 0,89
Recycled share in Recycled share in
Packaging kg %
material (kg) material (%)
Recycled
1,90 100,00 1,90 100,00
cardboard
Total incl.
9,44 100,00 2,79
packaging
Technical data:
Height 84 cm
Width 57 cm
Depth 58 cm
Weight 8 kg
Seat height 46 cm
Armrest height 64 cm
Seat width 41 cm
Max. user weight 160 kg
Market:
Europa
Reference service life, product
15 years
Reference service life, building
LCA: Calculation rules
Declared unit:
1 pcs Lake 01 stackable chair with armrest, upholstered, bolt base
Cut-off criteria:
All major raw materials and all the essential energy is included. The production processes for raw materials and energy flows with very small
amounts (less than 1%) are not included. These cut-off criteria do not apply for hazardous materials and substances.
All major raw materials and all the essential energy is included. The production processes for raw materials and energy flows with very small
amounts (less than 1%) are omitted. These cut-off criteria do not apply to hazardous materials and substances.
Cut-off criteria
Allocation:
The allocation is made in accordance with the provisions of EN 15804. Incoming energy and water and waste production in-house is allocated
equally among all products through mass allocation. Effects of primary production of recycled materials is allocated to the main product in which
the material was used. The recycling process and transportation of the material is allocated to this analysis.
3 / 12
Data quality:
Specific data for the product composition are provided by the manufacturer. They represent the production of the declared product and were
collected for EPD development in the year of study. Background data is based on registered EPDs according to EN 15804, Ostfold Research
databases, ecoinvent and other LCA databases. The data quality of the raw materials in A1 is presented in the table below.​
Materials Source Data quality Year
Metal - Steel ecoinvent 3.6 Database 2019
Plastic - Nylon (PA) ecoinvent 3.6 Database 2019
Plastic - Polyurethane (PUR) ecoinvent 3.6 Database 2019
Recycled cardboard Modified ecoinvent 3.6 Database 2019
Textile - Wool Modified ecoinvent 3.6 Database 2019
Wood - Plywood modified ecoinvent 3.6 Database 2019
4 / 12
System boundaries (X=included, MND=module not declared, MNR=module not relevant)
Construction Beyond the system
Product stage Use stage End of life stage
installation stage boundaries
A1 A2 A3 A4 A5 B1 B2 B3 B4 B5 B6 B7 C1 C2 C3 C4 D
X X X X X MND X X X MND MND MND X X X X MND
System boundary:
Additional technical information:
The Helland group is Norway's leading supplier of health and care furniture. Our unique combination of design, production, and sustainability has
set the quality standard for healthcare furniture for over 50 years. Helland has extensive cooperation with health institutions and furniture
designers in Scandinavia. Since its establishment in 1947, the company has had a head office in Stordal in Sunnmøre and established its own
production in Estonia in 2015. Helland products are sold in Norway, Sweden, and Germany. The Helland group is organized into two sales
companies, Helland Møbler AS (Sales in Norway, Sweden, and Denmark) and Helland Möbel GmbH (Eurozone customers). The Helland group has a
total of 70 employees.
Helland Møbler AS is certified according to EU regulations. We use the CO2 equivalent for hydropower.
Helland Møbler AS is certified according to the ISO-14001 standard.
Helland has launched several models with the Swan label, and these products are treated with a special water-based varnish. This varnish has a
high durability, but we advise against the use of disinfectants as this can shorten the life of the product. In addition, the Nordic Ecolabel will also
require that furniture textiles are used that either have the EU Ecolabel or the Nordic Ecolabel.
All our products are produced with FSC-approved wood. FSC is a global non-profit labeling scheme for wood and paper. In an FSC forest, no more
trees are felled than the forest can reproduce. At the same time, the FSC label is a guarantee that animals and plant life are protected and that the
people who work in the forest are guaranteed education, safety equipment, and regular pay conditions.
Helland Møbler has a modern production facility where a clean working environment is a high priority. Emissions from production that affect the
external and internal environment have been reduced to a minimum. The most commonly used types of wood are birch and oak, laminated and
solid wood. Chipboard, plywood, and solid wood are used for interior woodwork. All sheet material, as well as glue and varnish, satisfy the E-1
norm for formaldehyde release. Foam plastic is produced without the use of CFC gas. Environmentally friendly water-based contact adhesive is
used for gluing foam. All wood cladding is used for heating own premises. The cartons used are produced from recycled raw material. Cardboard,
paper, plastic, steel, electrical waste, and special waste are sorted and sent for recycling. Other waste is delivered to municipal landfills.
waR slairetam tropsnarT gnirutcafunaM tropsnarT ylbmessA e​sU ecnanetniaM riapeR tnemecalpeR tnemhsibrufeR lanoitarepO ygrene esu lanoitarepO esu retaw -eD noitcurtsnoc noitilomed tropsnarT etsaW gnissecorp lasopsiD -yrevoceR-esueR laitnetop-gnilcyceR
5 / 12
LCA: Scenarios and additional technical information
The following information describe the scenarios in the different modules of the EPD.
Capacity utilisation Value
Transport from production place to user (A4) Distance (km) Fuel/Energy Consumption Unit
(incl. return) % (Liter/tonne)
Truck, 16-32 tonnes, EURO 6 (km) 36,7 % 1000 0,043 l/tkm 43,00
Truck, 7.5-16 tonnes, EURO 6 (kgkm) 35,4 % 300 0,056 l/tkm 16,80
Assembly (A5) Unit Value
Waste, packaging, cardboard, 100 % recycled, to
kg 1,90
average treatment (kg)
Capacity utilisation Value
Transport to waste processing (C2) Distance (km) Fuel/Energy Consumption Unit
(incl. return) % (Liter/tonne)
Truck, 16-32 tonnes, EURO 6 (km) 36,7 % 85 0,043 l/tkm 3,66
Waste processing (C3) Unit Value
Waste treatment per kg Textile, incineration with
kg 0,70
fly ash extraction (kg)
Waste treatment per kg Plastics, Mixture,
kg 0,12
municipal incineration with fly ash extraction (kg)
Waste, materials to recycling (kg) kg 1,50
Waste treatment per kg Scrap steel, incineration
kg 4,43
with fly ash extraction (kg)
Waste treatment per kg Wood, incineration with
kg 1,50
fly ash extraction (kg)
Waste treatment per kg Polyurethane (PU),
kg 0,80
incineration (kg)
Disposal (C4) Unit Value
Landfilling of ashes from incineration of Textile,
kg 0,04
soiled, process per kg ashes and residues (kg)
Landfilling of ashes from incineration of Plastics,
Mixture, municipal incineration with fly ash
kg 0,00
extraction, process per kg ashes and residues - C4
(kg)
Landfilling of ashes and residues from
kg 2,93
incineration of Scrap steel (kg)
Landfilling of ashes from incineration of Wood,
kg 0,02
process per kg ashes and residues (kg)
Landfilling of ashes from incineration of
Polyurethane (PU), process per kg ashes and kg 0,03
residues - C4 (kg)
6 / 12
LCA: Results
The LCA results are presented below for the declared unit defined on page 2 of the EPD document.
Environmental impact
Indicator Unit A1-A3 A4 A5 B2 B3 B4 C1 C2 C3 C4
GWP-total
kg CO2 -
7,19E+01 2,15E+00 3,26E+00 0 0 0 0 1,31E-01 5,99E+00 3,48E-02
eq
GWP-fossil
kg CO2 -
5,31E+01 2,15E+00 3,07E-02 0 0 0 0 1,31E-01 2,47E+00 3,48E-02
eq
GWP-biogenic
kg CO2 -
1,56E+01 9,19E-04 3,23E+00 0 0 0 0 5,43E-05 3,52E+00 2,99E-05
eq
GWP-luluc
kg CO2 -
3,19E+00 8,11E-04 1,02E-05 0 0 0 0 4,67E-05 2,29E-05 1,02E-05
eq
kg
ODP CFC11 - 5,20E-06 4,82E-07 6,49E-09 0 0 0 0 2,97E-08 1,52E-08 1,03E-08
eq
mol H+
AP 1,00E+00 6,17E-03 1,46E-04 0 0 0 0 3,77E-04 2,39E-03 2,38E-04
-eq
EP-FreshWater kg P -eq 9,09E-03 1,79E-05 2,52E-07 0 0 0 0 1,05E-06 1,77E-06 3,54E-07
EP-Marine kg N -eq 1,74E-01 1,21E-03 4,81E-05 0 0 0 0 7,45E-05 1,28E-03 8,47E-05
mol N -
EP-Terrestial 3,73E+00 1,35E-02 5,21E-04 0 0 0 0 8,34E-04 1,25E-02 9,39E-04
eq
kg
POCP NMVOC 2,01E-01 5,17E-03 1,50E-04 0 0 0 0 3,19E-04 3,01E-03 2,70E-04
-eq
ADP- kg Sb-
7,71E-04 6,45E-05 7,48E-07 0 0 0 0 3,62E-06 6,45E-07 5,77E-07
minerals&metals1 eq
ADP-fossil1 MJ 6,41E+02 3,24E+01 4,30E-01 0 0 0 0 1,98E+00 1,31E+00 7,67E-01
WDP1 m3 3,37E+03 3,34E+01 5,45E-01 0 0 0 0 1,92E+00 3,69E+00 1,67E+00
GWP-total = Global Warming Potential total; GWP-fossil = Global Warming Potential fossil fuels; GWP-biogenic = Global Warming Potential biogenic; GWP-luluc =
Global Warming Potential land use and land use change; ODP = Depletion potential of the stratospheric ozone layer; AP = Acidification potential, Accumulated
Exceedance; EP-freshwater = Eutrophication potential, fraction of nutrients reaching freshwater end compartment: EP-marine = Eutrophication potential, fraction of
nutrients reaching marine end compartment; EP-terrestrial = Eutrophication potential, Accumulated Exceedance; POCP = Formation potential of tropospheric ozone;
ADP-minerals&metals = Abiotic depletion potential for non-fossil resources; ADP-fossil = Abiotic depletion for fossil resources potential; WDP = Water (user)
deprivation potential, deprivation-weighted water consumption
"Reading example: 9,0 E-03 = 9,0*10-3 = 0,009"
*INA Indicator Not Assessed
1. The results of this environmental impact indicator shall be used with care as the uncertainties on these results are high or as there is limited experienced with the
indicator
Remarks to environmental impacts
7 / 12
Additional environmental impact indicators
Indicator Unit A1-A3 A4 A5 B2 B3 B4 C1 C2 C3 C4
PM Disease incidence 8,56E-06 1,28E-07 2,15E-09 0 0 0 0 8,03E-09 1,71E-08 4,32E-09
IRP2 kgBq U235 -eq 2,82E+00 1,42E-01 1,84E-03 0 0 0 0 8,66E-03 2,37E-03 3,08E-03
ETP-fw1 CTUe 1,65E+03 2,43E+01 5,73E-01 0 0 0 0 1,47E+00 8,14E+00 4,76E-01
HTP-c1 CTUh 1,34E-07 0,00E+00 1,80E-11 0 0 0 0 0,00E+00 4,33E-10 1,80E-11
HTP-nc1 CTUh 1,31E-06 2,74E-08 7,20E-10 0 0 0 0 1,61E-09 1,13E-08 4,83E-10
SQP1 dimensionless -2,78E+04 2,17E+01 2,88E-01 0 0 0 0 1,39E+00 1,80E-01 1,68E+00
PM = Particulate Matter emissions; IRP = Ionizing radiation – human health; ETP-fw = Eco toxicity – freshwater; HTP-c = Human toxicity – cancer effects; HTP-nc =
Human toxicity – non cancer effects; SQP = Soil Quality (dimensionless)
"Reading example: 9,0 E-03 = 9,0*10-3 = 0,009"
*INA Indicator Not Assessed
1. The results of this environmental impact indicator shall be used with care as the uncertainties on these results are high or as there is limited experienced with the
indicator
2. This impact category deals mainly with the eventual impact of low dose ionizing radiation on human health of the nuclear fuel cycle. It does not consider effects due
to possible nuclear accidents, occupational exposure nor due to radioactive waste disposal in underground facilities. Potential ionizing radiation from the soil, from
radon and from some construction materials is also not measured by this indicator.
8 / 12
Resource use
Indicator Unit A1-A3 A4 A5 B2 B3 B4 C1 C2 C3 C4
PERE MJ 2,32E+02 4,88E-01 7,08E-03 0 0 0 0 2,84E-02 4,22E-02 1,50E-02
PERM MJ 4,75E+01 0,00E+00 -1,11E+01 0 0 0 0 0,00E+00 -3,64E+01 0,00E+00
PERT MJ 2,80E+02 4,88E-01 -1,11E+01 0 0 0 0 2,84E-02 -3,63E+01 1,50E-02
PENRE MJ 6,36E+02 3,24E+01 4,30E-01 0 0 0 0 1,98E+00 1,32E+00 7,67E-01
PENRM MJ 2,90E+01 0,00E+00 0,00E+00 0 0 0 0 0,00E+00 -2,90E+01 0,00E+00
PENRT MJ 6,65E+02 3,24E+01 4,30E-01 0 0 0 0 1,98E+00 -2,77E+01 7,67E-01
SM kg 2,79E+00 0,00E+00 0,00E+00 0 0 0 0 0,00E+00 0,00E+00 0,00E+00
RSF MJ 5,81E-01 1,75E-02 2,35E-04 0 0 0 0 1,02E-03 9,55E-04 3,95E-04
NRSF MJ 3,26E-01 6,29E-02 9,68E-04 0 0 0 0 3,63E-03 0,00E+00 2,51E-02
FW m3 5,56E-01 3,57E-03 2,03E-04 0 0 0 0 2,12E-04 4,13E-03 6,92E-04
PERE = Use of renewable primary energy excluding renewable primary energy resources used as raw materials; PERM = Use of renewable primary energy resources used
as raw materials; PERT = Total use of renewable primary energy resources; PENRE = Use of non renewable primary energy excluding non-renewable primary energy
resources used as raw materials; PENRM = Use of non renewable primary energy resources used as raw materials; PENRT = Total use of non renewable primary energy
resources; SM = Use of secondary materials; RSF = Use of renewable secondary fuels; NRSF = Use of non-renewable secondary fuels; FW = Net use of fresh water
"Reading example: 9,0 E-03 = 9,0*10-3 = 0,009"
*INA Indicator Not Assessed
9 / 12
End of life - Waste
Indicator Unit A1-A3 A4 A5 B2 B3 B4 C1 C2 C3 C4
HWD kg 3,71E-01 1,70E-03 0,00E+00 0 0 0 0 1,02E-04 0,00E+00 2,95E+00
NHWD kg 9,38E+00 1,49E+00 1,90E+00 0 0 0 0 9,64E-02 0,00E+00 4,50E-02
RWD kg 2,84E-03 2,20E-04 0,00E+00 0 0 0 0 1,35E-05 0,00E+00 4,70E-06
HWD = Hazardous waste disposed; NHWD = Non-hazardous waste disposed; RWD = Radioactive waste disposed
"Reading example: 9,0 E-03 = 9,0*10-3 = 0,009"
*INA Indicator Not Assessed
End of life - Output flow
Indicator Unit A1-A3 A4 A5 B2 B3 B4 C1 C2 C3 C4
CRU kg 0,00E+00 0,00E+00 0,00E+00 0 0 0 0 0,00E+00 0,00E+00 0,00E+00
MFR kg 5,31E-02 0,00E+00 1,77E+00 0 0 0 0 0,00E+00 1,50E+00 0,00E+00
MER kg 6,02E-01 0,00E+00 2,59E-06 0 0 0 0 0,00E+00 7,54E+00 0,00E+00
EEE MJ 3,53E-01 0,00E+00 1,09E-01 0 0 0 0 0,00E+00 2,95E+00 0,00E+00
EET MJ 5,34E+00 0,00E+00 1,64E+00 0 0 0 0 0,00E+00 4,46E+01 0,00E+00
CRU = Components for re-use; MFR = Materials for recycling; MER = Materials for energy recovery; EEE = Exported energy electrical; EET = Exported energy thermal
"Reading example: 9,0 E-03 = 9,0*10-3 = 0,009"
*INA Indicator Not Assessed
Biogenic Carbon Content
Indicator Unit At the factory gate
Biogenic carbon content in product kg C 6,82E-01
Biogenic carbon content in accompanying packaging kg C 8,80E-01
Note: 1 kg biogenic carbon is equivalent to 44/12 kg CO2
10 / 12
Additional requirements
Greenhouse gas emissions from the use of electricity in the manufacturing phase
National production mix from import, low voltage (production of transmission lines, in addition to direct emissions and losses in grid) of applied
electricity for the manufacturing process (A3).
Electricity mix Source Amount Unit
Electricity, Estonia (kWh) ecoinvent 3.6 926,93 g CO2-eq/kWh
Dangerous substances
The product contains no substances given by the REACH Candidate list.
Indoor environment
Our Furniture does not contain any substances that affect indoor climate.
Additional Environmental Information
Key Environmental Indicators
Key environmental indicators Unit A1-A3 A4 A1-C4 A1-D
GWPtotal kg CO2 -eq 71,92 2,15 83,49 83,49
Total energy consumption MJ 868,82 32,94 906,38 906,38
Amount of recycled materials % 29,51
Additional environmental impact indicators required in NPCR Part A for construction products
Indicator Unit A1-A3 A4 A5 B2 B3 B4 C1 C2 C3 C4
GWPIOBC kg CO2 -eq 7,89E+01 2,15E+00 3,07E-02 0 0 0 0 1,31E-01 3,61E+00 3,74E-02
GWP-IOBC: Global warming potential calculated according to the principle of instantaneous oxidation. In order to increase the transparency of biogenic carbon
contribution to climate impact, the indicator GWP-IOBC is required as it declares climate impacts calculated according to the principle of instantaneous oxidation.
GWP-IOBC is also referred to as GWP-GHG in context to Swedish public procurement legislation.
Variants and Options
Key environmental indicators (A1-A3) for variants of this EPD
Variants
Weight GWPtotal (kg CO2 -
Total energy consumption (MJ)Amount of recycled materials (%)
(kg) eq)
Lake 01 stackable chair without armrest, upholstered, bolt
8,20 68,98 813,59 25,86
base
11 / 12
Bibliography
ISO 14025:2010 Environmental labels and declarations - Type III environmental declarations - Principles and procedures.
ISO 14044:2006 Environmental management - Life cycle assessment - Requirements and guidelines.
EN 15804:2012+A2:2019 Environmental product declaration - Core rules for the product category of construction products.
ISO 21930:2017 Sustainability in buildings and civil engineering works - Core rules for environmental product declarations of construction
products.
ecoinvent v3, Allocation, cut-off by classification, Swiss Centre of Life Cycle Inventories.
Iversen et al., (2021) eEPD v2021.09 Background information for EPD generator tool system verification, LCA.no Report number: 07.21
Ruud et al., (2023) EPD generator for NPCR026 Part B for Furniture - Background information for EPD generator application and LCA data,
LCA.no report number 01.23
NPCR Part A: Construction products and services. Ver. 2.0. March 2021, EPD-Norge.
NPCR 026 Part B for Furniture. Ver. 2.0 March 2022, EPD-Norge.
Program operator and publisher Phone: +47 977 22 020
The Norwegian EPD Foundation e-mail: post@epd-norge.no
Post Box 5250 Majorstuen, 0303 Oslo, Norway web: www.epd-norge.no
Owner of the declaration: Phone: +47 958 09 013
Helland Møbler AS e-mail: joakim.helland@helland.no
Postboks 10, 6259 Stordal, Norway web: www.helland.no
Author of the Life Cycle Assessment Phone: +47 916 50 916
LCA.no AS e-mail: post@lca.no
Dokka 6A, 1671 Kråkerøy, Norway web: www.lca.no
Developer of EPD generator Phone: +47 916 50 916
LCA.no AS e-mail: post@lca.no
Dokka 6A, 1671 Kråkerøy, Norway web: www.lca.no
ECO Platform web: www.eco-platform.org
ECO Portal web: ECO Portal
12 / 12
