Environmental product declaration
in accordance with ISO 14025 and EN 15804+A2
FLEXRÖR 20/FQ Pure 6G1,5mm² 5T
Owner of the declaration: Program operator:
Prysmian Group Sverige AB The Norwegian EPD Foundation
Product: Declaration number:
FLEXRÖR 20/FQ Pure 6G1,5mm² 5T
Registration number:
Declared unit:
1 m Issue date:
This declaration is based on Product Category Rules: Valid to:
CEN Standard EN 15804:2012+A2:2019 serves as core
EPD software:
PCR
The Norwegian EPD Foundation LCAno EPD generator ID: 212236
NPCR 027:2020 Part B for Electrical cables and wires
1 / 12
General information
Product Owner of the declaration:
FLEXRÖR 20/FQ Pure 6G1,5mm² 5T Prysmian Group Sverige AB
Contact person: Anders Sjöland
Phone: +46 706128204
e-mail: anders.sjoland@prysmiangroup.com
Program operator: Manufacturer:
The Norwegian EPD Foundation Prysmian Group Sverige AB
Post Box 5250 Majorstuen, 0303 Oslo, Norway Vallgatan 5
Phone: +47 977 22 020 571 41 Nässjö, Sweden
web: www.epd-norge.no
Declaration number: Place of production:
Prysmian Group production site Emmen (Netherlands)
Abel Tasmanstraat 1
7821 AN Emmen, Netherlands
This declaration is based on Product Category Rules: Management system:
CEN Standard EN 15804:2012+A2:2019 serves as core PCR ISO 9001, ISO 14001, ISO 45001
NPCR 027:2020 Part B for Electrical cables and wires
Statement of liability: Organisation no:
The owner of the declaration shall be liable for the underlying 556556-2104
information and evidence. EPD Norway shall not be liable with respect
to manufacturer information, life cycle assessment data and
evidences.​
Declared unit: Issue date:
1 m FLEXRÖR 20/FQ Pure 6G1,5mm² 5T
Declared unit with option: Valid to:
A1,A2,A3,A4,A5,C1,C2,C3,C4,D
Year of study:
2022
Functional unit: Comparability:
1 m of FLEXRÖR 20/FQ Pure 6G1,5mm² electrical cable, installed EPD of construction products may not be comparable if they not
open or piped in indoor installations, with a reference service life of comply with EN 15804 and seen in a building context.
30 years.
General information on verification of EPD from EPD tools: Development and verification of EPD:
Independent verification of data, other environmental information The declaration is created using EPD tool lca.tools ver EPD2022.03,
and the declaration according to ISO 14025:2010, § 8.1.3 and § 8.1.4. developed by LCA.no. The EPD tool is integrated in the company's
Verification of each EPD is made according to EPD-Norway’s management system, and has been approved by EPD Norway.
guidelines for verification and approval requiring that tools are i) Approval number: NEPDT33
integrated into the company's environmental management system, ii)
the procedures for use of the EPD tool are approved by EPD-Norway, Developer of EPD: Siri Andersen
and iii) the process is reviewed annually by an independent third
Reviewer of company-specific input data and EPD:​ Anders Nymark
party verifier. See Appendix G of EPD-Norway's General Programme
Instructions for further information on EPD tools
Verification of EPD tool: Approved:
Independent third party verification of the EPD tool, background data
and test-EPD in accordance with EPDNorway's procedures and
guidelines for verification and approval of EPD tools. Approval
number: NEPDT32.
Third party verifier:
Vito D’Incognito, Take Care International
(no signature required)
2 / 12
Product
Product description:
Flex pipes in halogen-free PP (Polypropylene) with Draka’s quality cable FQ Pure, which is part of Prysmian Group’s Eco Cable concept that helps
our customers in their environmental work.
To reduce the product’s carbon footprint, the cable consists of 36% recycled copper. The cable meets CPR class Dca s2d2a1. Approved for casting,
stiffness class 750 N and with impact resistance up to 2 kg. UV and ozone resistant, which provides a long service life.
The cable inside is like Draka’s other high-quality cables and is easy to work with.
Product specification
Conductor material Copper
Conductor surface Bare
Core insulation material Low smoke zero halogen polymer
Tube material Halogen-free PP
Twisted cores Yes
Materials kg %
HFFR Polyolefin 0,05 25,32
Metal - Copper 0,08 39,67
Plastic - Polyethylene 0,00 0,17
Plastic - Polypropylene (PP) 0,07 34,84
Total 0,19 100,00
Technical data:
FLEXRÖR 20/FQ Pure 6G1,5mm²
SAP code: 20434796
External article code: 1419823
SS-EN 50525-3-31 Construction standard
Reaction-to-fire class (acc. EN 13501-6) Dca
Smoke development class (acc. EN 13501-6) s2
Euro class flaming droplets/particles (acc. EN 13501-6) d2
Euro class acidity (acc. EN 13501-6) a1
Market:
Sweden
Reference service life, product
30 years. Standard lifetime for residential/tertiary/industrial building applications, provided in appendix 1 of PSR for wires, cables, and accessories
of PEP Ecopassport.
Reference service life, building or construction works
30 years. Estimation made to match the product service life and keep the EPD environmental impact calculations at the product level.
LCA: Calculation rules
Declared unit:
1 m FLEXRÖR 20/FQ Pure 6G1,5mm² 5T
Cut-off criteria:
All major raw materials and all the essential energy is included. The production processes for raw materials and energy flows with very small
amounts (less than 1%) are not included. These cut-off criteria do not apply for hazardous materials and substances.
Allocation:
The allocation is made in accordance with the provisions of EN 15804. Incoming energy and water and waste production in-house is allocated
equally among all products through mass allocation. Effects of primary production of recycled materials is allocated to the main product in which
the material was used. The recycling process and transportation of the material is allocated to this analysis.
Data quality:
Specific data for the product composition are provided by the manufacturer. The data represent the production of the declared product and were
collected for EPD development in the year of study. Background data is based on EPDs according to EN 15804 and different LCA databases. The
data quality of the raw materials in A1 is presented in the table below.
3 / 12
Materials Source Data quality Year
HFFR Polyolefin ecoinvent 3.6 Database 2019
Metal - Copper Modified ecoinvent 3.6 Database 2019
Plastic - Polyethylene ecoinvent 3.6 Database 2019
Plastic - Polypropylene (PP) ecoinvent 3.6 Database 2019
4 / 12
System boundaries (X=included, MND=module not declared, MNR=module not relevant)
Construction Beyond the system
Product stage Use stage End of life stage
installation stage boundaries
A1 A2 A3 A4 A5 B1 B2 B3 B4 B5 B6 B7 C1 C2 C3 C4 D
X X X X X MND MND MND MND MND MND MND X X X X X
System boundary:
The flowchart below illustrates the system boundaries of the analysis:
Additional technical information:
waR slairetam tropsnarT gnirutcafunaM tropsnarT ylbmessA e​sU ecnanetniaM riapeR tnemecalpeR tnemhsibrufeR lanoitarepO ygrene esu lanoitarepO esu retaw -eD noitcurtsnoc noitilomed tropsnarT etsaW gnissecorp lasopsiD -yrevoceR-esueR laitnetop-gnilcyceR
5 / 12
LCA: Scenarios and additional technical information
The following information describe the scenarios in the different modules of the EPD.
Module A4 = An average distance between the factory in Emmen and the Swedish market is considered.
Installation (A5) and removal (C1) is assumed to be done with other products such as piping systems and should be assessed at a contruction
works level.
For B1-B7 the default environmental impact and resource indicators in the EPD are assumed to be zero.
In C2, a distance of 300 km has been added as average transport to nearest waste treatment facilities.
In C3, datasets are developed for the recycling of metals and plastics and for the incinerations of plastic fractions (including energy recovery and
fly ash extraction). All other minor raw materials in the product are assumed to be incinerated. Net benefit of material recycling and energy
recovery are given in module D.
Capacity utilisation Value
Transport from production place to user (A4) Distance (km) Fuel/Energy Consumption Unit
(incl. return) % (Liter/tonne)
Truck, over 32 tonnes, EURO 5 (km) 53,3 % 1500 0,023 l/tkm 34,50
Assembly (A5) Unit Value
Product loss during installation (percentage of
Units/DU 0,02
cable)
Capacity utilisation Value
Transport to waste processing (C2) Distance (km) Fuel/Energy Consumption Unit
(incl. return) % (Liter/tonne)
Truck, 16-32 tonnes, EURO 5 (km) 36,7 % 300 0,044 l/tkm 13,20
Waste processing (C3) Unit Value
Copper to recycling (kg) kg 0,05
Polypropylene (PP) to recycling (kg) kg 0,01
Waste treatment of plastic mixture, incineration
kg 0,02
with energy recovery and fly ash extraction (kg)
Waste treatment of polyethylene (PE),
incineration with energy recovery and fly ash kg 0,00
extraction (kg)
Waste treatment of polypropylene (PP),
incineration with energy recovery and fly ash kg 0,03
extraction (kg)
Disposal (C4) Unit Value
Landfilling of ashes from incineration of Plastic
kg 0,00
mixture, process per kg ashes and residues (kg)
Landfilling of ashes from incineration of
Polyethylene (PE), process per kg ashes and kg 0,00
residues (kg)
Landfilling of ashes from incineration of
Polypropylene (PP), process per kg ashes and kg 0,00
residues (kg)
Landfilling of copper (kg) kg 0,03
Landfilling of plastic mixture (kg) kg 0,05
Benefits and loads beyond the system
Unit Value
boundaries (D)
Substitution of electricity (MJ) MJ 0,08
Substitution of Polypropylene, PP granulate (kg) kg 0,01
Substitution of primary copper with net scrap (kg) kg 0,02
Substitution of thermal energy, district heating
MJ 1,24
(MJ)
6 / 12
LCA: Results
The LCA results are presented below for the declared unit defined on page 2 of the EPD document.
Environmental impact
Indicator Unit A1 A2 A3 A4 A5 C1 C2 C3 C4 D
GWP-total
kg CO2 -
5,24E-01 3,70E-03 4,57E-02 2,64E-02 1,49E-02 0 9,67E-03 1,27E-01 6,38E-03 -7,80E-02
eq
GWP-fossil
kg CO2 -
5,20E-01 3,70E-03 4,43E-02 2,63E-02 1,47E-02 0 9,67E-03 1,27E-01 6,38E-03 -7,74E-02
eq
GWP-biogenic
kg CO2 -
3,18E-03 1,52E-06 1,39E-03 1,08E-05 9,18E-05 0 3,94E-06 1,83E-06 5,50E-07 -3,38E-04
eq
GWP-luluc
kg CO2 -
5,18E-04 1,08E-06 7,26E-05 7,69E-06 1,21E-05 0 3,38E-06 3,22E-07 2,93E-07 -3,00E-04
eq
kg
ODP CFC11 - 2,87E-08 8,54E-10 3,80E-09 6,09E-09 8,42E-10 0 2,20E-09 1,80E-10 2,88E-10 -5,22E-04
eq
mol H+
AP 2,86E-02 1,55E-05 1,91E-04 1,11E-04 5,79E-04 0 3,95E-05 2,14E-05 7,57E-06 -7,53E-03
-eq
EP-FreshWater kg P -eq 2,42E-04 2,82E-08 3,32E-06 2,01E-07 4,92E-06 0 7,59E-08 1,70E-08 1,39E-08 -5,08E-05
EP-Marine kg N -eq 1,22E-03 4,67E-06 2,82E-05 3,33E-05 2,63E-05 0 1,17E-05 1,02E-05 8,83E-06 -3,38E-04
mol N -
EP-Terrestial 1,76E-02 5,17E-05 3,19E-04 3,68E-04 3,72E-04 0 1,30E-04 1,07E-04 3,03E-05 -5,08E-03
eq
kg
POCP NMVOC 5,37E-03 1,66E-05 8,31E-05 1,18E-04 1,13E-04 0 3,97E-05 2,58E-05 9,84E-06 -1,42E-03
-eq
ADP- kg Sb-
8,37E-05 6,39E-08 2,38E-07 4,50E-07 1,69E-06 0 2,62E-07 8,87E-09 7,51E-09 -4,17E-05
minerals&metals1 eq
ADP-fossil1 MJ 1,02E+01 5,75E-02 7,65E-01 4,10E-01 2,32E-01 0 1,46E-01 1,26E-02 2,24E-02 -1,44E+00
WDP1 m3 1,69E+01 4,43E-02 9,59E+00 3,14E-01 5,49E-01 0 1,39E-01 6,84E-02 3,68E-01 3,55E-01
GWP-total = Global Warming Potential total; GWP-fossil = Global Warming Potential fossil fuels; GWP-biogenic = Global Warming Potential biogenic; GWP-luluc =
Global Warming Potential land use and land use change; ODP = Depletion potential of the stratospheric ozone layer; AP = Acidification potential, Accumulated
Exceedance; EP-freshwater = Eutrophication potential, fraction of nutrients reaching freshwater end compartment: EP-marine = Eutrophication potential, fraction of
nutrients reaching marine end compartment; EP-terrestrial = Eutrophication potential, Accumulated Exceedance; POCP = Formation potential of tropospheric ozone;
ADP-minerals&metals = Abiotic depletion potential for non-fossil resources; ADP-fossil = Abiotic depletion for fossil resources potential; WDP = Water (user)
deprivation potential, deprivation-weighted water consumption
"Reading example: 9,0 E-03 = 9,0*10-3 = 0,009"
*INA Indicator Not Assessed
1. The results of this environmental impact indicator shall be used with care as the uncertainties on these results are high or as there is limited experienced with the
indicator
Remarks to environmental impacts
7 / 12
Additional environmental impact indicators
Indicator Unit A1 A2 A3 A4 A5 C1 C2 C3 C4 D
PM Disease incidence 6,22E-08 3,24E-10 5,48E-10 2,32E-09 1,33E-09 0 6,96E-10 9,70E-11 1,41E-10 -1,91E-08
IRP2 kgBq U235 -eq 1,99E-02 2,51E-04 5,64E-03 1,79E-03 5,67E-04 0 6,37E-04 2,82E-05 1,27E-04 -1,61E-03
ETP-fw1 CTUe 2,32E+02 4,21E-02 4,88E-01 3,00E-01 5,04E+00 0 1,07E-01 1,36E-01 1,90E+01 -6,86E+01
HTP-c1 CTUh 4,69E-09 0,00E+00 1,60E-11 0,00E+00 9,40E-11 0 0,00E+00 5,00E-12 1,00E-12 -9,74E-10
HTP-nc1 CTUh 3,88E-07 4,00E-11 4,96E-10 2,90E-10 7,78E-09 0 1,16E-10 2,11E-10 2,50E-11 -8,28E-08
SQP1 dimensionless 4,43E+00 6,55E-02 1,63E-01 4,70E-01 1,06E-01 0 1,00E-01 2,04E-03 6,36E-02 -1,57E+00
PM = Particulate Matter emissions; IRP = Ionizing radiation – human health; ETP-fw = Eco toxicity – freshwater; HTP-c = Human toxicity – cancer effects; HTP-nc =
Human toxicity – non cancer effects; SQP = Potential Soil Quality Index (dimensionless)
"Reading example: 9,0 E-03 = 9,0*10-3 = 0,009"
*INA Indicator Not Assessed
1. The results of this environmental impact indicator shall be used with care as the uncertainties on these results are high or as there is limited experienced with the
indicator
2. This impact category deals mainly with the eventual impact of low dose ionizing radiation on human health of the nuclear fuel cycle. It does not consider effects due
to possible nuclear accidents, occupational exposure nor due to radioactive waste disposal in underground facilities. Potential ionizing radiation from the soil, from
radon and from some construction materials is also not measured by this indicator.
8 / 12
Resource use
Indicator Unit A1 A2 A3 A4 A5 C1 C2 C3 C4 D
PERE MJ 1,01E+00 7,26E-04 1,24E-01 5,16E-03 2,30E-02 0 2,06E-03 5,85E-04 1,99E-03 -8,04E-01
PERM MJ 0,00E+00 0,00E+00 0,00E+00 0,00E+00 0,00E+00 0 0,00E+00 0,00E+00 0,00E+00 0,00E+00
PERT MJ 1,01E+00 7,26E-04 1,24E-01 5,16E-03 2,30E-02 0 2,06E-03 5,85E-04 1,99E-03 -8,04E-01
PENRE MJ 7,45E+00 5,75E-02 7,66E-01 4,10E-01 1,77E-01 0 1,46E-01 1,26E-02 2,24E-02 -1,05E+00
PENRM MJ 2,93E+00 0,00E+00 0,00E+00 0,00E+00 5,26E-04 0 0,00E+00 -2,91E+00 0,00E+00 -4,33E-01
PENRT MJ 1,04E+01 5,75E-02 7,66E-01 4,10E-01 1,78E-01 0 1,46E-01 -2,89E+00 2,24E-02 -1,48E+00
SM kg 2,87E-02 0,00E+00 0,00E+00 0,00E+00 5,77E-04 0 0,00E+00 0,00E+00 1,59E-04 1,29E-02
RSF MJ 8,38E-03 2,54E-05 9,00E-03 1,80E-04 3,54E-04 0 7,36E-05 1,34E-05 4,14E-05 3,72E-04
NRSF MJ 1,56E-03 8,53E-05 2,24E-03 6,05E-04 9,75E-05 0 2,63E-04 0,00E+00 1,18E-04 -3,50E-02
FW m3 2,00E-02 6,54E-06 6,52E-04 4,67E-05 4,18E-04 0 1,53E-05 8,03E-05 2,85E-05 -2,11E-03
PERE = Use of renewable primary energy excluding renewable primary energy resources used as raw materials; PERM = Use of renewable primary energy resources used
as raw materials; PERT = Total use of renewable primary energy resources; PENRE = Use of non renewable primary energy excluding non-renewable primary energy
resources used as raw materials; PENRM = Use of non renewable primary energy resources used as raw materials; PENRT = Total use of non renewable primary energy
resources; SM = Use of secondary materials; RSF = Use of renewable secondary fuels; NRSF = Use of non-renewable secondary fuels; FW = Net use of fresh water
"Reading example: 9,0 E-03 = 9,0*10-3 = 0,009"
*INA Indicator Not Assessed
9 / 12
End of life - Waste
Indicator Unit A1 A2 A3 A4 A5 C1 C2 C3 C4 D
HWD kg 3,83E-03 3,14E-06 2,65E-03 2,24E-05 1,67E-04 0 7,43E-06 0,00E+00 1,86E-03 -5,18E-04
NHWD kg 1,13E-01 4,96E-03 4,50E-03 3,57E-02 4,96E-03 0 6,97E-03 0,00E+00 8,31E-02 -2,44E-02
RWD kg 1,73E-05 3,93E-07 4,66E-06 2,80E-06 5,26E-07 0 9,94E-07 0,00E+00 1,52E-07 -1,38E-06
HWD = Hazardous waste disposed; NHWD = Non-hazardous waste disposed; RWD = Radioactive waste disposed
"Reading example: 9,0 E-03 = 9,0*10-3 = 0,009"
*INA Indicator Not Assessed
End of life - Output flow
Indicator Unit A1 A2 A3 A4 A5 C1 C2 C3 C4 D
CRU kg 0,00E+00 0,00E+00 0,00E+00 0,00E+00 0,00E+00 0 0,00E+00 0,00E+00 0,00E+00 0,00E+00
MFR kg 0,00E+00 0,00E+00 1,11E-04 0,00E+00 1,19E-03 0 0,00E+00 5,95E-02 4,91E-06 -5,11E-04
MER kg 0,00E+00 0,00E+00 1,03E-02 0,00E+00 1,24E-03 0 0,00E+00 5,16E-02 3,99E-06 -9,82E-05
EEE MJ 0,00E+00 0,00E+00 6,05E-03 0,00E+00 1,76E-03 0 0,00E+00 8,18E-02 4,17E-05 -2,18E-04
EET MJ 0,00E+00 0,00E+00 9,16E-02 0,00E+00 2,66E-02 0 0,00E+00 1,24E+00 6,31E-04 -3,30E-03
CRU = Components for re-use; MFR = Materials for recycling; MER = Materials for energy recovery; EEE = Exported energy electrical; EET = Exported energy thermal
"Reading example: 9,0 E-03 = 9,0*10-3 = 0,009"
*INA Indicator Not Assessed
Biogenic Carbon Content
Indicator Unit At the factory gate
Biogenic carbon content in product kg C 0,00E+00
Biogenic carbon content in accompanying packaging kg C 0,00E+00
Note: 1 kg biogenic carbon is equivalent to 44/12 kg CO2
10 / 12
Additional requirements
Greenhouse gas emissions from the use of electricity in the manufacturing phase
National production mix from import, low voltage (production of transmission lines, in addition to direct emissions and losses in grid) of applied
electricity for the manufacturing process (A3).
Electricity mix Source Amount Unit
Electricity, European average (kWh) ecoinvent 3.6 428,03 g CO2-eq/kWh
Dangerous substances
The product contains no substances given by the REACH Candidate list.
Indoor environment
Additional Environmental Information
Additional environmental impact indicators required in NPCR Part A for construction products
Indicator Unit A1 A2 A3 A4 A5 C1 C2 C3 C4 D
GWPIOBC kg CO2 -eq 5,15E-01 3,70E-03 4,76E-02 2,64E-02 1,47E-02 0 9,67E-03 1,27E-01 6,54E-03 -5,28E-02
GWP-IOBC: Global warming potential calculated according to the principle of instantaneous oxidation. In order to increase the transparency of biogenic carbon​
contribution to climate impact, the indicator GWP-IOBC is required as it declares climate impacts calculated according to the principle of instantaneous oxidation.​
GWP-IOBC is also referred to as GWP-GHG in context to Swedish public procurement legislation.
11 / 12
Bibliography
ISO 14025:2010. Environmental labels and declarations - Type III environmental declarations - Principles and procedures. International
Organization for Standardization.
ISO 14044:2006. Environmental management - Life cycle assessment - Requirements and guidelines. International Organization for
Standardization.
EN 15804:2012+A2:2019. Environmental product declaration - Core rules for the product category of construction products. European
Committee for Standardization.
ISO 21930:2017. Sustainability in buildings and civil engineering works - Core rules for environmental product declarations of construction
products. International Organization for Standardization.
EN 50693:2019. Product category rules for life cycle assessments of electronic and electrical products and systems. European Committee for
Standardization.
Ecoinvent v3, 2019. Allocation, cut-off by classification. Swiss Centre of Life Cycle Inventories.
Iversen et al., (2021). eEPD v2021.09, background information for EPD generator tool system verification, LCA.no. Report number: 07.21. System
verification report.
Philis et al., (2022). EPD generator for NPCR 027 part B for electrical wires and cables, background information for EPD generator application and
LCA data, LCA.no Report number: 03.22. PCR verification report.
EPD Norway (2022). NPCR Part A: Construction products and services. The Norwegian EPD foundation. Version 2.0 published 24.03.2021.
EPD Norway (2022). NPCR 027 Part B for electrical cables and wires. The Norwegian EPD foundation. Version 2.0 published 01.03.2022.
Program operator and publisher Phone: +47 977 22 020
The Norwegian EPD Foundation e-mail: post@epd-norge.no
Post Box 5250 Majorstuen, 0303 Oslo, Norway web: www.epd-norge.no
Owner of the declaration: Phone: +46 706128204
Prysmian Group Sverige AB e-mail: anders.sjoland@prysmiangroup.com
Vallgatan 5, 571 41 Nässjö web:
Author of the Life Cycle Assessment Phone: +47 916 50 916
LCA.no AS e-mail: post@lca.no
Dokka 6B, 1671 web: www.lca.no
Developer of EPD generator Phone: +47 916 50 916
LCA.no AS e-mail: post@lca.no
Dokka 6B,1671 Kråkerøy web: www.lca.no
ECO Platform web: www.eco-platform.org
ECO Portal web: ECO Portal
12 / 12
