Environmental product declaration
in accordance with ISO 14025 and EN 15804+A2
Lyssand 120 Side-hung window with two opening sashes, wood, 1230x1480
Owner of the declaration: Program operator:
Lyssand-Frekhaug AS The Norwegian EPD Foundation
Product: Declaration number:
Lyssand 120 Side-hung window with two opening sashes,
wood, 1230x1480 NEPD-9239-8826
Declared unit: Registration number:
1 pcs
NEPD-9239-8826
This declaration is based on Product Category Rules:
Issue date: 26.02.2025
CEN Standard EN 15804:2012+A2:2019 serves as core
The Norwegian EPD Foundation PCR Valid to: 26.02.2030
NPCR 014:2019 Part B for Windows and doors
EPD software:
LCAno EPD generator ID: 796110
1 / 13
General information
Product Owner of the declaration:
Lyssand 120 Side-hung window with two opening sashes, wood, Lyssand-Frekhaug AS
1230x1480 Contact person: Christian Tollefsen
Phone: +47 56 30 33 00
e-mail: firmapost@lf-as.no
Program operator: Manufacturer:
The Norwegian EPD Foundation Lyssand-Frekhaug AS
Post Box 5250 Majorstuen, 0303 Oslo, Norway
Phone: +47 977 22 020
web: www.epd-norge.no
Declaration number: Place of production:
Lyssand-Frekhaug AS
NEPD-9239-8826 Ulsmågveien 7
5224 Nesttun, Norway
This declaration is based on Product Category Rules: Management system:
CEN Standard EN 15804:2012+A2:2019 serves as core PCR
NPCR 014:2019 Part B for Windows and doors
Statement of liability: Organisation no:
The owner of the declaration shall be liable for the underlying 988381063
information and evidence. EPD Norway shall not be liable with respect
to manufacturer information, life cycle assessment data and
evidences.​
Declared unit: Issue date:
1 pcs Lyssand 120 Side-hung window with two opening sashes,
26.02.2025
wood, 1230x1480
Declared unit with option: Valid to:
A1-A3,A4,A5,B2,B4,C1,C2,C3,C4,D 26.02.2030
Year of study:
2022
Functional unit: Comparability:
A wooden side-hung window with a triple glazed insulating glass. Two EPD of construction products may not be comparable if they not
opening sashes that opens outwards. The weight of the finished comply with EN 15804 and seen in a building context.
window is 38,08 kg per m².
General information on verification of EPD from EPD tools: Development and verification of EPD:
Independent verification of data, other environmental information The declaration is created using EPD tool lca.tools ver EPD2022.03,
and the declaration according to ISO 14025:2010, § 8.1.3 and § 8.1.4. developed by LCA.no. The EPD tool is integrated in the company's
Verification of each EPD is made according to EPD-Norway’s management system, and has been approved by EPD Norway.
guidelines for verification and approval requiring that tools are i)
integrated into the company's environmental management system, ii) Developer of EPD: Christian Tollefsen
the procedures for use of the EPD tool are approved by EPD-Norway,
Reviewer of company-specific input data and EPD:​ Gudmund
and iii) the process is reviewed annually by an independent third
Osmundsen
party verifier. See Appendix G of EPD-Norway's General Programme
Instructions for further information on EPD tools
Verification of EPD tool: Approved:
Independent third party verification of the EPD tool, background data
and test-EPD in accordance with EPDNorway's procedures and
guidelines for verification and approval of EPD tools.
Third party verifier:
Gaylord K. Booto, Norwegian Institute for Air Research (NILU)
(no signature required)
2 / 13
Product
Product description:
Wooden window used in building facades.
Product specification
Wooden frame and sashes made from finger jointed Pine, vacuum impregnated at factory for long service life. Painted with primer and top coat.
Materials kg %
Adhesive and sealant 0,06 0,09
Metal - Galvanized Steel 0,17 0,24
Metal - Steel low alloy 0,19 0,27
Paint, water-based 2,40 3,47
Plastic - Polypropylene (PP) 0,11 0,15
Plastic - Polyvinyl chloride (PVC) 1,33 1,92
Rubber, synthetic 0,13 0,19
Triple glazing 37,03 53,38
Wood preservative 0,70 1,01
Metal 0,21 0,31
Metal - Aluminium 0,62 0,90
Metal - Steel 0,88 1,27
Chemical 0,13 0,18
Plastic - Polyurethane (PUR) 0,14 0,20
Wood 0,02 0,03
Wood - Laminated wood 25,26 36,41
Total 69,37 100,00
Packaging kg %
Packaging - Cardboard 0,30 8,99
Packaging - Plastic 0,18 5,39
Packaging - Wood 2,86 85,62
Total incl. packaging 72,70 100,00
Technical data:
120 mm deep wooden frame.
48mm Triple glazed insulating glass unit (IGU, 4-18-4-18-4) with a warm edge spacer and Argon filled cavities. Both the inner and outer glass
panes are coated with low emission coating. U-value for declared unit is 0,92.
Area of functional unit is 1230x1480mm, 1,82m², conversion factor is 0,549 for 1m².
The production is approved by NDVK (Norsk dør- og vinduskontroll) All timber used is certified FSC or PEFC with full traceability.
Market:
Norway
Reference service life, product
40 years
For the windows expected life length to be realised, it is paramount that instructions for assembly and care provided by the manufacturer are
followed.
Reference service life, building or construction works
60 years
LCA: Calculation rules
Declared unit:
1 pcs Lyssand 120 Side-hung window with two opening sashes, wood, 1230x1480
Cut-off criteria:
All major raw materials and all the essential energy is included. The production processes for raw materials and energy flows with very small
amounts (less than 1%) are not included. These cut-off criteria do not​ apply for hazardous materials and substances.
Allocation:
The allocation is made in accordance with the provisions of EN 15804. Effects of primary production of recycled materials is allocated to the main
product in which the material was used. The recycling process and transportation of the material is allocated to this analysis. The PCR specific
background data follow the allocation rules in the Ecoinvent v3.7.1 Cut-off database version. The allocation of water, energy and waste flows
within the production facilities for windows and doors follows unit-based allocation adjusted with a point system to different product groups or
products. This score system is regulated by a factor which increases with the resource intensity of each product. The unit-based allocation is
adjusted by the weight of the product, excluding the weight of glass.
Data quality:
3 / 13
Specific data for the product composition are provided by the manufacturer. The data represent the production of the declared product and were
collected for EPD development in the year of study. Background data is based on EPDs according to EN 15804 and different LCA databases. The
data quality of the raw materials in A1 is presented in the table below.
Materials Source Data quality Year
Adhesive and sealant EPD-DBC-20220147-IBF1-EN EPD 2021
Adhesive and sealant EPD-FEI-20220021-IBG1-EN EPD 2021
Chemical ecoinvent 3.6 Database 2019
Metal EPD-ARG-20230542-IBG1-EN EPD 2022
Metal - Aluminium ecoinvent 3.6 Database 2019
Metal - Aluminium S-P-07377 EPD 2021
Metal - Galvanized Steel Ecoinvent 3.6 Database 2019
Metal - Steel ecoinvent 3.6 Database 2019
Metal - Steel low alloy ecoinvent 3.6 Database 2019
Packaging - Cardboard ecoinvent 3.6 Database 2019
Packaging - Plastic ecoinvent 3.6 Database 2019
Packaging - Wood Modified ecoinvent 3.6 Database 2019
Paint, water-based ecoinvent 3.6 Database 2019
Plastic - Polypropylene (PP) ecoinvent 3.6 Database 2019
Plastic - Polyurethane (PUR) ecoinvent 3.6 Database 2019
Plastic - Polyvinyl chloride (PVC) ecoinvent 3.6 Database 2019
Rubber, synthetic ecoinvent 3.6 Database 2019
Triple glazing EPD-MIG-GB-61.0 EPD 2020
Wood modified ecoinvent 3.6 Database 2019
Wood - Laminated wood EPD HUB, HUB-0100 EPD 2023
Wood preservative ecoinvent 3.6 Database 2019
4 / 13
System boundaries (X=included, MND=module not declared, MNR=module not relevant)
Construction Beyond the system
Product stage Use stage End of life stage
installation stage boundaries
A1 A2 A3 A4 A5 B1 B2 B3 B4 B5 B6 B7 C1 C2 C3 C4 D
X X X X X MND X MND X MND MND MND X X X X X
System boundary:
Additional technical information:
waR slairetam tropsnarT gnirutcafunaM tropsnarT ylbmessA e​sU ecnanetniaM riapeR tnemecalpeR tnemhsibrufeR lanoitarepO ygrene esu lanoitarepO esu retaw -eD noitcurtsnoc noitilomed tropsnarT etsaW gnissecorp lasopsiD -yrevoceR-esueR laitnetop-gnilcyceR
5 / 13
LCA: Scenarios and additional technical information
The following information describe the scenarios in the different modules of the EPD.
Conditions and scenarios for user data in EPD phases
A4
Transportation is assumed at 300km from factory site in Frekhaug Norway. Transported using a large EURO 6 truck with delivery directly to
construction site.
A5
As the product installation can vary from different construction sites, height of the building and other unknown factors, the installation is assumed
to be done manually and no other parameters are considered for this calculation. Waste treatment of packaging is included in the EPD
calculations.
B2/B3
Maintenance is included as cleaning 3 times pr year and lubricating metal parts. As the IGUhas an RSL of 30 years, it is assumed that the whole
window would be replaced after 30 years rather than just the IGU. No repairs are assumed during RSL.
B4/B5
The windows reference service life (RSL) is estimatet at 40 years, there is assumed no refurbishment needed during RSL, apart from what is
included in B2/B3.
B6
The product has no operational energy use.
C1
It is assumed that the window will be manually deconstructed for recycling and waste, hence no energy usage is assumed for this. The window is
assumed to be treated as mixed waste and sent to incineration. Glass is assumed to go to landfill and metals are sorted from the ash and recycled.
C2
It is assumed a transport from deconstruction to waste/incineration of 50km.
Capacity utilisation Value
Transport from production place to user (A4) Distance (km) Fuel/Energy Consumption Unit
(incl. return) % (Liter/tonne)
Lastebil med henger, over 32 tonn, EURO 6 (km) 53,3 % 300 0,023 l/tkm 6,90
Assembly (A5) Unit Value
Waste, packaging, pallet, EUR wooden pallet,
kg 2,85
reusable, average treatment (kg)
Waste, packaging, corrugated board box, to
kg 0,30
average treatment (kg)
Waste, packaging, plastic film (LDPE), to average
kg 0,18
treatment (kg)
Maintenance (B2) Unit Value
Treatment of wastewater (kg) kg 126,000000000
Soap solution 5%, household detergent (kg) kg 6,000000000
Lubricating oil (kg) kg 0,20
Water, tap water (kg) kg 120,000000000
Replacement (B4) Unit Value
Replacement of product including waste
Units 1,000000000
treatment (pcs)
Capacity utilisation Value
Transport to waste processing (C2) Distance (km) Fuel/Energy Consumption Unit
(incl. return) % (Liter/tonne)
Lastebil, 7.5-16 tonn, EURO 6 (km) 35,4 % 50 0,056 l/tkm 2,80
Waste processing (C3) Unit Value
Waste treatment per kg Wood, from incineration
kg 23,77
(kg)
Waste treatment per kg Paint, hazardous waste
kg 2,28
incineration (kg)
Waste treatment per kg Rubber, municipal
kg 0,12
incineration with fly ash extraction (kg)
Waste treatment per kg Polypropylene, PP,
kg 0,10
incineration with fly ash extraction (kg)
Materials to recycling (kg) kg 13,071
Waste treatment per kg Polyurethane (PU),
kg 0,13
incineration (kg)
Waste treatment per kg Non-hazardous waste,
kg 1,084
incineration with fly ash extraction (kg)
Waste treatment per kg Polyvinylchloride (PVC),
kg 1,26
incineration with fly ash extraction (kg)
6 / 13
Disposal (C4) Unit Value
Waste, wood, to landfill (kg) kg 1,25
Landfilling of ashes from incineration of
Polyurethane (PU), process per kg ashes and kg 0,0050
residues (kg)
Landfilling of ashes from incineration of Non-
hazardous waste, process per kg ashes and
kg 0,25
residues (kg)
Waste, glass, to landfill, sanitary landfill (kg) kg 25,91
Waste, municipal solid waste, to landfill (kg) kg 0,057
Landfilling of ashes from incineration of Wood,
kg 0,27
process per kg ashes and residues (kg)
Landfilling of ashes from incineration of
Polyvinylchloride (PVC), process per kg ashes and kg 0,20
residues (kg)
Waste, polyurethane, to landfill (kg) kg 0,0070
Waste, scrap aluminium, to landfill (kg) kg 0,041
Landfilling of ashes from incineration of
Polypropylene, PP, process per kg ashes and kg 0,0030
residues (kg)
Waste, rubber, to landfill (kg) kg 0,0065
Waste, paint, to landfill (kg) kg 0,12
Landfilling of ashes from incineration of Rubber,
kg 0,0064
process per kg ashes and residues (kg)
Waste, scrap steel, to landfill (kg) kg 0,061
Waste, polyvinylchloride, to landfill (kg) kg 0,066
Waste, polypropylene, to landfill (kg) kg 0,0053
Landfilling of ashes from incineration of Paint,
hazardous waste incineration, process of ashes kg 0,067
and residues (kg)
Benefits and loads beyond the system
Unit Value
boundaries (D)
Substitution of electricity, in Norway (MJ) MJ 19,10
Substitution of primary glass with net scrap (kg) kg 9,29
Substitution of thermal energy, district heating, in
MJ 289,046
Norway (MJ)
Substitution of primary steel with net scrap (kg) kg 0,78
Substitution of primary aluminium with net scrap
kg 0,67
(kg)
7 / 13
LCA: Results
The LCA results are presented below for the declared unit defined on page 2 of the EPD document.
Environmental impact
Indicator Unit A1-A3 A4 A5 B2 B4 C1 C2 C3 C4 D
GWP-total
kg CO2 -
7,05E+01 1,81E+00 4,86E+00 2,01E+00 0,00E+00 0 7,44E-01 5,55E+01 5,09E-01 -1,82E+01
eq
GWP-fossil
kg CO2 -
1,13E+02 1,81E+00 2,30E-02 9,53E-01 0,00E+00 0 7,43E-01 1,38E+01 3,58E-01 -1,79E+01
eq
GWP-biogenic
kg CO2 -
-4,58E+01 7,77E-04 4,84E+00 1,28E-01 0,00E+00 0 3,44E-04 4,17E+01 1,51E-01 -1,21E-01
eq
GWP-luluc
kg CO2 -
3,05E+00 5,52E-04 3,68E-06 9,34E-01 0,00E+00 0 3,21E-04 9,88E-04 8,63E-05 -1,75E-01
eq
kg
ODP CFC11 - 8,33E-06 4,37E-07 2,50E-09 2,54E-07 0,00E+00 0 1,63E-07 5,74E-07 9,40E-08 -1,22E-01
eq
mol H+
AP 1,19E+00 5,84E-03 7,15E-05 1,04E-02 0,00E+00 0 2,13E-03 1,23E-02 2,55E-03 -1,58E-01
-eq
EP-FreshWater kg P -eq 1,51E-02 1,44E-05 1,15E-07 4,91E-03 0,00E+00 0 6,81E-06 2,60E-05 4,59E-06 -6,00E-04
EP-Marine kg N -eq 2,09E-01 1,28E-03 3,69E-05 1,07E-02 0,00E+00 0 4,04E-04 3,67E-03 1,00E-03 -2,61E-02
mol N -
EP-Terrestial 2,37E+00 1,43E-02 2,87E-04 3,09E-02 0,00E+00 0 4,54E-03 3,99E-02 9,71E-03 -3,05E-01
eq
kg
POCP NMVOC 6,21E-01 5,60E-03 8,09E-05 9,96E-03 0,00E+00 0 1,73E-03 1,12E-02 2,82E-03 -8,33E-02
-eq
ADP- kg Sb-
3,10E-03 3,23E-05 2,56E-07 6,10E-05 0,00E+00 0 2,68E-05 1,36E-05 3,10E-06 -8,23E-04
minerals&metals1 eq
ADP-fossil1 MJ 2,04E+03 2,94E+01 1,72E-01 1,96E+01 0,00E+00 0 1,11E+01 3,42E+01 6,91E+00 -2,08E+02
WDP1 m3 4,07E+03 2,26E+01 3,63E-01 6,13E+01 0,00E+00 0 1,33E+01 1,87E+02 1,35E+01 -3,78E+03
GWP-total = Global Warming Potential total; GWP-fossil = Global Warming Potential fossil fuels; GWP-biogenic = Global Warming Potential biogenic; GWP-luluc =
Global Warming Potential land use and land use change; ODP = Depletion potential of the stratospheric ozone layer; AP = Acidification potential, Accumulated
Exceedance; EP-freshwater = Eutrophication potential, fraction of nutrients reaching freshwater end compartment: EP-marine = Eutrophication potential, fraction of
nutrients reaching marine end compartment; EP-terrestrial = Eutrophication potential, Accumulated Exceedance; POCP = Formation potential of tropospheric ozone;
ADP-minerals&metals = Abiotic depletion potential for non-fossil resources; ADP-fossil = Abiotic depletion for fossil resources potential; WDP = Water (user)
deprivation potential, deprivation-weighted water consumption
"Reading example: 9,0 E-03 = 9,0*10-3 = 0,009"
*INA Indicator Not Assessed
1. The results of this environmental impact indicator shall be used with care as the uncertainties on these results are high or as there is limited experienced with the
indicator
Remarks to environmental impacts
8 / 13
Additional environmental impact indicators
Indicator Unit A1-A3 A4 A5 B2 B4 C1 C2 C3 C4 D
PM Disease incidence 1,12E-05 1,67E-07 1,03E-09 1,30E-07 0,00E+00 0 4,16E-08 2,05E-07 4,85E-08 -2,31E-06
IRP2 kgBq U235 -eq 8,74E+00 1,29E-01 7,20E-04 7,38E-02 0,00E+00 0 4,85E-02 1,57E-01 2,80E-02 -7,24E-01
ETP-fw1 CTUe 4,57E+03 2,15E+01 1,98E-01 1,10E+02 0,00E+00 0 8,65E+00 2,04E+02 3,19E+01 -4,69E+02
HTP-c1 CTUh 1,72E-07 0,00E+00 1,00E-11 2,18E-09 0,00E+00 0 0,00E+00 1,74E-08 2,40E-10 -2,39E-08
HTP-nc1 CTUh 3,22E-06 2,08E-08 4,41E-10 5,23E-08 0,00E+00 0 1,04E-08 1,14E-07 5,76E-09 -2,80E-07
SQP1 dimensionless 1,13E+03 3,38E+01 1,73E-01 3,96E+01 0,00E+00 0 6,60E+00 1,62E+01 1,86E+01 -2,09E+02
PM = Particulate Matter emissions; IRP = Ionizing radiation – human health; ETP-fw = Eco toxicity – freshwater; HTP-c = Human toxicity – cancer effects; HTP-nc =
Human toxicity – non cancer effects; SQP = Potential Soil Quality Index (dimensionless)
"Reading example: 9,0 E-03 = 9,0*10-3 = 0,009"
*INA Indicator Not Assessed
1. The results of this environmental impact indicator shall be used with care as the uncertainties on these results are high or as there is limited experienced with the
indicator
2. This impact category deals mainly with the eventual impact of low dose ionizing radiation on human health of the nuclear fuel cycle. It does not consider effects due
to possible nuclear accidents, occupational exposure nor due to radioactive waste disposal in underground facilities. Potential ionizing radiation from the soil, from
radon and from some construction materials is also not measured by this indicator.
9 / 13
Resource use
Indicator Unit A1-A3 A4 A5 B2 B4 C1 C2 C3 C4 D
PERE MJ 8,31E+02 3,70E-01 3,53E-03 9,35E+00 0,00E+00 0 1,89E-01 6,86E+00 1,27E-01 -1,81E+02
PERM MJ 2,78E+02 0,00E+00 -4,21E+01 0,00E+00 0,00E+00 0 0,00E+00 -2,36E+02 0,00E+00 0,00E+00
PERT MJ 1,11E+03 3,70E-01 -4,21E+01 9,35E+00 0,00E+00 0 1,89E-01 -2,29E+02 1,27E-01 -1,81E+02
PENRE MJ 1,96E+03 2,94E+01 1,72E-01 2,08E+01 0,00E+00 0 1,11E+01 3,44E+01 6,91E+00 -2,08E+02
PENRM MJ 8,69E+01 0,00E+00 -7,64E+00 0,00E+00 0,00E+00 0 0,00E+00 -7,92E+01 0,00E+00 0,00E+00
PENRT MJ 2,05E+03 2,94E+01 -7,47E+00 2,08E+01 0,00E+00 0 1,11E+01 -4,49E+01 6,91E+00 -2,08E+02
SM kg 2,42E+00 0,00E+00 0,00E+00 2,47E-03 0,00E+00 0 0,00E+00 0,00E+00 0,00E+00 0,00E+00
RSF MJ 1,22E+00 1,30E-02 1,03E-04 2,17E-02 0,00E+00 0 6,81E-03 1,41E-01 2,74E-03 -6,03E-03
NRSF MJ 2,80E+00 4,34E-02 5,63E-04 2,72E-02 0,00E+00 0 2,47E-02 0,00E+00 1,40E-01 -7,83E+00
FW m3 2,77E+00 3,35E-03 9,60E-05 1,13E-01 0,00E+00 0 1,32E-03 9,13E-02 7,46E-03 -3,83E-01
PERE = Use of renewable primary energy excluding renewable primary energy resources used as raw materials; PERM = Use of renewable primary energy resources used
as raw materials; PERT = Total use of renewable primary energy resources; PENRE = Use of non renewable primary energy excluding non-renewable primary energy
resources used as raw materials; PENRM = Use of non renewable primary energy resources used as raw materials; PENRT = Total use of non renewable primary energy
resources; SM = Use of secondary materials; RSF = Use of renewable secondary fuels; NRSF = Use of non-renewable secondary fuels; FW = Net use of fresh water
"Reading example: 9,0 E-03 = 9,0*10-3 = 0,009"
*INA Indicator Not Assessed
10 / 13
End of life - Waste
Indicator Unit A1-A3 A4 A5 B2 B4 C1 C2 C3 C4 D
HWD kg 8,02E-01 1,61E-03 0,00E+00 9,95E-02 0,00E+00 0 6,14E-04 0,00E+00 4,48E-01 -1,49E-02
NHWD kg 7,37E+01 2,56E+00 6,23E-01 3,02E-01 0,00E+00 0 4,38E-01 1,08E+00 2,80E+01 -3,29E+00
RWD kg 4,49E-02 2,01E-04 0,00E+00 9,48E-05 0,00E+00 0 7,48E-05 0,00E+00 4,26E-06 -7,63E-04
HWD = Hazardous waste disposed; NHWD = Non-hazardous waste disposed; RWD = Radioactive waste disposed
"Reading example: 9,0 E-03 = 9,0*10-3 = 0,009"
*INA Indicator Not Assessed
End of life - Output flow
Indicator Unit A1-A3 A4 A5 B2 B4 C1 C2 C3 C4 D
CRU kg 0,00E+00 0,00E+00 2,71E+00 0,00E+00 0,00E+00 0 0,00E+00 0,00E+00 0,00E+00 0,00E+00
MFR kg 1,61E+00 0,00E+00 3,71E-01 1,74E-03 0,00E+00 0 0,00E+00 1,31E+01 1,12E-04 0,00E+00
MER kg 1,41E+00 0,00E+00 1,63E-01 5,69E-05 0,00E+00 0 0,00E+00 2,65E+01 2,32E-06 0,00E+00
EEE MJ 8,59E-01 0,00E+00 1,16E-01 3,46E-04 0,00E+00 0 0,00E+00 1,83E+01 1,76E-04 0,00E+00
EET MJ 1,30E+01 0,00E+00 1,75E+00 5,23E-03 0,00E+00 0 0,00E+00 2,78E+02 2,66E-03 0,00E+00
CRU = Components for re-use; MFR = Materials for recycling; MER = Materials for energy recovery; EEE = Exported energy electrical; EET = Exported energy thermal
"Reading example: 9,0 E-03 = 9,0*10-3 = 0,009"
*INA Indicator Not Assessed
Biogenic Carbon Content
Indicator Unit At the factory gate
Biogenic carbon content in product kg C 1,14E+01
Biogenic carbon content in accompanying packaging kg C 1,32E+00
Note: 1 kg biogenic carbon is equivalent to 44/12 kg CO2
11 / 13
Additional requirements
Greenhouse gas emissions from the use of electricity in the manufacturing phase
National production mix from import, low voltage (production of transmission lines, in addition to direct emissions and losses in grid) of applied
electricity for the manufacturing process (A3).
Electricity mix Source Amount Unit
Electricity, Norway (kWh) ecoinvent 3.6 24,33 g CO2-eq/kWh
Dangerous substances
The product contains no substances on the REACH Candidate list at or above 100 ppm, 0,01 % by weight.
Indoor environment
No known emissions.
Additional Environmental Information
Additional environmental impact indicators required in NPCR Part A for construction products
Indicator Unit A1-A3 A4 A5 B2 B4 C1 C2 C3 C4 D
GWPIOBC kg CO2 -eq 1,17E+02 1,81E+00 2,30E-02 2,01E+00 0,00E+00 0 7,43E-01 1,27E+01 5,14E-01 -1,83E+01
GWP-IOBC: Global warming potential calculated according to the principle of instantaneous oxidation. In order to increase the transparency of biogenic carbon​
contribution to climate impact, the indicator GWP-IOBC is required as it declares climate impacts calculated according to the principle of instantaneous oxidation.​
GWP-IOBC is also referred to as GWP-GHG in context to Swedish public procurement legislation.
12 / 13
Bibliography
ISO 14025:2010 Environmental labels and declarations - Type III environmental declarations - Principles and procedures.
ISO 14044:2006 Environmental management - Life cycle assessment - Requirements and guidelines.
EN 15804:2012+A2:2019 Environmental product declaration - Core rules for the product category of construction products.
ISO 21930:2017 Sustainability in buildings and civil engineering works - Core rules for environmental product declarations of construction
products.
ecoinvent v3, Allocation, cut-off by classification, Swiss Centre of Life Cycle Inventories.
Iversen et al., (2021) eEPD v2021.09 Background information for EPD generator tool system verification, LCA.no Report number: 07.21
Iversen et al., (2022) EPD generator for EPD generator for NPCR 014
Part B for Windows and doors, Background information for EPD generator application and LCA data, LCA.no report number: 17.22
NPCR Part A: Construction products and services. Ver. 2.0. April 2021, EPD-Norge.
NPCR 014 Part B for Windows and doors, Ver. 4.0, 20.09.2021, EPD Norway.
Program operator and publisher Phone: +47 977 22 020
The Norwegian EPD Foundation e-mail: post@epd-norge.no
Post Box 5250 Majorstuen, 0303 Oslo, Norway web: www.epd-norge.no
Owner of the declaration: Phone: +47 56 30 33 00
Lyssand-Frekhaug AS e-mail: firmapost@lf-as.no
Ulsmågveien 7, 5224 Nesttun, Norway web: www.lyssand.com
Author of the Life Cycle Assessment Phone: +47 916 50 916
LCA.no AS e-mail: post@lca.no
Dokka 6A, 1671 Kråkerøy, Norway web: www.lca.no
Developer of EPD generator Phone: +47 916 50 916
LCA.no AS e-mail: post@lca.no
Dokka 6A, 1671 Kråkerøy, Norway web: www.lca.no
ECO Platform web: www.eco-platform.org
ECO Portal web: ECO Portal
13 / 13
