ver1 2015
ENVIRONMENTAL PRODUCT DECLARATION
in accordance with ISO 14025, ISO 21930 and EN 15804
Owner of the declaration: Elektroskandia Norge AS
Program operator: The Norwegian EPD Foundation
Publisher: The Norwegian EPD Foundation
Declaration number: NEPD-3360-1989-EN
Registration number: NEPD-3360-1989-EN
ECO Platform reference number: -
Issue date: 16.02.2022
Valid to: 16.02.2027
3G2,5 PFXP-LX-ER WHITE
Elektroskandia Norge AS
www.epd-norge.no
NEPD-3360-1989-EN 3G2,5 PFXP-LX-ER WHITE (ver2-040422) 1 / 8
General information
Product: Owner of the declaration:
3G2,5 PFXP-LX-ER WHITE Elektroskandia Norge AS
Contact person: Pål Kristiansen
Phone: +47 97 66 22 12
e-mail: pkr@elektroskandia.no
Program operator: Manufacturer:
NKT AS
The Norwegian EPD Foundation
Støperigata 7 3040 Drammen
Pb. 5250 Majorstuen, 0303 Oslo
Norway
Phone: +47 23 08 80 00
e-mail: post@epd-norge.no
Declaration number: Place of production:
NKT (Denmark) A/S
NEPD-3360-1989-EN Toftegårdsvej 25 DK-4550 Asnæs
Denmark
ECO Platform reference number: Management system:
ISO 14001, ISO 9001
This declaration is based on Product Category Rules: Organisation no:
977 454 700
CEN Standard EN 15804:2012+A1:2013 serves as core PCR
NPCR 027 Part B for Electrical cables and wires
Statement of liability: Issue date:
The owner of the declaration shall be liable for the underlying information and 16.02.2022
evidence. EPD Norway shall not be liable with respect to manufacturer
information, life cycle assessment data and evidences. Valid to:
16.02.2027
Declared unit: Year of study:
1 m 3G2,5 PFXP-LX-ER WHITE 2020
Declared unit with option: Comparability:
EPD of construction products may not be comparable if they not comply with EN
A1,A2,A3,A4,C1,C2,C3,C4,D
15804 and seen in a building context.
Functional unit: Development and verification of EPD:
1 m of 3G2,5 PFXP-LX electrical cable installed in open installations and The declaration has been developed and verified using EPD tool lca.tools
pipes from cradle-to-grave with with a reference service life of 80 years ver EPD2020.11, developed by LCA.no AS. The EPD tool is integrated into
the company's environmental management system, and has been
approved by EPD-Norway
General information on verification of EPD from EPD tools:
Independent verification of data, other environmental information and Developer of EPD:
the declaration according to ISO 14025:2010, § 8.1.3 and § 8.1.4. Individual
third party verification of each EPD is not required when the EPD tool is i) Preben Hansen, NKT as
integrated into the company's environmental management system, ii) the
procedures for use of the EPD tool are approved by EPDNorway, and iii) Reviewer of company-specific input data and EPD:
the proccess is reviewed annualy. See Appendix G of EPD-Norway's
General Programme Instructions for further information on EPD tools. Marco Mezzadra
Verification of EPD tool: Approved:
Independent third party verification of the EPD tool, background data
Sign
and test-EPD in accordance with EPDNorway's procedures and guidelines
for verification and approval of EPD tools.
Fredrik Moltu Johnsen, Norsus AS
(no signature required) Håkon Hauan, CEO EPD-Norge
NEPD-3360-1989-EN 3G2,5 PFXP-LX-ER WHITE (ver2-040422) 2 / 8
Product
Product description: Technical data:
For fixed installation in open installations and pipes. Standard: NKT factory standard 014
The cable is double insulated. Can be laid in the ground if extra Solid or stranded, round copper conductor
protection is provided. The conductor insulation must be protected XLPE insulation
against UV radiation. Filling sheat, lead-free PVC
This EPD represent the entire product family of the Building wire Outer sheat, lead-free PVC
"300/500V PFXP-LX ER". This EPD is for our most sold product. Contact Test voltage: 2 kV AC
us for the specific EPD of other cables within this product family Rated voltage: 300/500 V
(product references are listed under the additional technical Max. conductor temperature: 70 °C
information) Max. short-circuit temperature: 250 °C
Min. handling temperature: -5 °C
Product specification
Bending radius: 5 x D
Building wire 300/500V CPR fire class: Eca
PFXP-LX-ER WHITE Colour of sheath: White
Fulfills the low voltage directive: Yes
Market:
Materials kg %
Norway
E-PVC 0,07 49,07
Copper 0,06 44,02 Reference service life, product
Polyethylene 0,01 6,91
80 years
Total: 0,14
Reference service life, construcion
100 years
LCA: Calculation rules
Declared unit: Allocation:
The allocation is made in accordance with the provisions of EN 15804.
1 m 3G2,5 PFXP-LX-ER WHITE
Incoming energy and water and waste production in-house is allocated
Cut-off criteria: equally among all products through mass allocation. Effects of primary
production of recycled materials is allocated to the main product in which
All major raw materials and all the essential energy is included. The
the material was used. The recycling process and transportation of the
production processes for raw materials and energy flows with very small
material is allocated to this analysis.
amounts (less than 1%) are not included. These cut-off criteria do not
apply for hazardous materials and substances.
Data quality:
Specific data for the product composition are provided by the manufacturer. They represent the production of the declared product and were collected for
EPD development in the year of study. Background data is based on registered EPDs according to EN 15804, Ostfold Research databases, ecoinvent and other
LCA databases. The data quality of the raw materials in A1 is presented in the table below.
Materials Source Data quality Year
Copper ecoinvent 3.6 Database 2019
E-PVC ecoinvent 3.6 Database 2019
Polyethylene ecoinvent 3.6 Database 2019
NEPD-3360-1989-EN 3G2,5 PFXP-LX-ER WHITE (ver2-040422) 3 / 8
System boundary:
Additional technical information:
This EPD is for our most sold product, contact us for the specific EPD of other cables within this family.
Building wire 300/500V PFXP-LX ER.
All the different products are specified in the this paragraph.
PFXP-LX ER
3G1,5 B/100 1056520
3G1,5 T/300 1056530
4G1,5 B/100 1056521
4G1,5 T/300 1056531
5G1,5 B/100 1056522
5G1,5 T/250 1056532
3G2,5 B/50 1056523
3G2,5 T/250 1056533
4G2,5 B/50 1056524
4G2,5 T/250 1056534
5G2,5 B/50 1056525
5G2,5 T/200 1056535
PFXP-LX FR
3G1,5 B/100 1056540
3G1,5 T/300 1056550
4G1,5 B/100 1056541
4G1,5 T/300 1056551
5G1,5 B/50 1056542
5G1,5 T/250 1056552
3G2,5 B/50 1056543
3G2,5 T/250 1056553
4G2,5 B/50 1056544
4G2,5 T/250 1053554
5G2,5 B/50 1056545
5G2,5 T/200 1056555
NEPD-3360-1989-EN 3G2,5 PFXP-LX-ER WHITE (ver2-040422) 4 / 8
LCA: Scenarios and additional technical information
The following information describe the scenarios in the different modules of the EPD.
The following information describe the scenarios in the different modules of the EPD. In A4, a transport distance of 669 km from the NKT Group production
site in Denmark to Elektroskandia’s warehouse in Langhus was included. 300 km was also added as additional transport to market. Installation in trenches (A5)
and removal (C1) is assumed to be done with other products such as piping systems and should be assessed at a construction works level. For B1-B7 the
default environmental impact and resource indicators in the EPD are assumed to be zero. Some other potential environmental impacts from the use phase
might not be covered by the scope of an EPD. In C3 metals such as copper are sent to recycling, like vice cross-linked polyethylene is reused in other cable
industry applications, finally other plastic materials are sent to municipal incineration. Net benefit of material recycling and energy recovery is given in module
D.
Transport from production place to user (A4)
Capacity utilisation Fuel/Energy
Type Type of vehicle Distance km Unit Value (l/t)
(incl. return) % consumption
Truck 38,8 % Truck, lorry 16-32 tonnes, EURO 4 969 0,044575 l/tkm 43,19
Railway l/tkm
Boat l/tkm
Other Transportation l/tkm
End of Life (C1, C3, C4)
. Unit Value
Hazardous waste disposed kg
Collected as mixed construction waste kg
Reuse kg
Recycling kg 0,0573
Energy recovery kg 0,0810
To landfill kg 0,0092
Transport to waste processing (C2)
Capacity utilisation Fuel/Energy
Type Type of vehicle Distance km Unit Value (l/t)
(incl. return) % consumption
Truck 38,8 % Truck, lorry 16-32 tonnes, EURO 6 85 0,043626 l/tkm 3,71
Railway l/tkm
Boat l/tkm
Other Transportation l/tkm
¨
Benefits and loads beyond the system boundaries (D)
. Unit Value
Substitution of primary Copper with net secondary copper (kg) kg 0,04
Substitution of electricity, in Norway (MJ) MJ 0,30
Substitution of thermal energy, district heating, in Norway (MJ) MJ 2,05
NEPD-3360-1989-EN 3G2,5 PFXP-LX-ER WHITE (ver2-040422) 5 / 8
LCA: Results
LCA results according to the indicators of EN 15804:2013+A1:2013 are presented in the following tables, for the declared unit defined on page 2 of the EPD
document. All potential environmental impacts might not be covered by the EN 15804 indicators. This concerns indicators such as noise, electromagnetic
radiation, electromagnetic fields and treatment brominated flame retardants.
System boundaries (X=included, MND=module not declared, MNR=module not relevant)
Construction Beyond the
Product stage installation User stage End of life stage . system
stage bondaries
A1 A2 A3 A4 A5 B1 B2 B3 B4 B5 B6 B7 C1 C2 C3 C4 . D
X X X X MND MND MND MND MND MND MND MND X X X X . X
Environmental impact
Parameter Unit A1-A3 A4 C1 C2 C3 C4 D
GWP kg CO 2 -eq 7,35E-01 2,26E-02 0 1,96E-03 1,86E-01 5,04E-04 -9,80E-02
ODP kg CFC11 -eq 1,16E-07 4,21E-09 0 3,69E-10 2,93E-09 3,80E-11 -8,83E-09
POCP kg C 2H 4-eq 1,56E-03 3,71E-06 0 2,97E-07 3,25E-06 5,80E-08 -7,81E-04
AP kg SO 2 -eq 4,05E-02 8,79E-05 0 4,61E-06 5,09E-05 1,23E-06 -1,98E-02
EP kg PO 3- -eq 2,31E-03 1,58E-05 0 6,05E-07 9,34E-06 2,05E-07 -9,22E-04
4
ADPM kg Sb -eq 5,30E-07 6,95E-08 0 6,09E-09 3,51E-08 4,00E-12 -1,77E-07
ADPE MJ 9,64E+00 3,43E-01 0 2,96E-02 1,12E-01 3,57E-03 -1,23E+00
GWP Global warming potential; ODP Depletion potential of the stratospheric ozone layer; POCP Formation potential of tropospheric photochemical oxidants;
AP Acidification potential of land and water; EP Eutrophication potential; ADPM Abiotic depletion potential for non fossil resources; ADPE Abiotic depletion
potential for fossil resources
"Reading example: 9,0 E-03 = 9,0*10-3 = 0,009"
*INA Indicator Not Assessed
waR slairetam tropsnarT gnirutcafunaM tropsnarT ylbmessA esU ecnanetniaM riapeR tnemecalpeR tnemhsibrufeR lanoitarepO ygrene esu lanoitarepO esu
retaw
-eD noitcurtsnoc noitilomed tropsnarT etsaW gnissecorp lasopsiD -yrevoceR-esueR -gnilcyceR laitnetop
NEPD-3360-1989-EN 3G2,5 PFXP-LX-ER WHITE (ver2-040422) 6 / 8
Resource use
Parameter Unit A1-A3 A4 C1 C2 C3 C4 D
RPEE MJ 1,59E+00 5,01E-03 0 4,37E-04 1,55E-02 2,55E-04 -1,17E+00
RPEM MJ 0,00E+00 0,00E+00 0 0,00E+00 0,00E+00 0,00E+00 0,00E+00
TPE MJ 1,59E+00 5,01E-03 0 4,37E-04 1,55E-02 2,55E-04 -1,17E+00
NRPE MJ 8,80E+00 3,52E-01 0 3,03E-02 1,28E-01 3,91E-03 -1,58E+00
NRPM MJ 1,93E+00 0,00E+00 0 0,00E+00 0,00E+00 0,00E+00 0,00E+00
TRPE MJ 1,07E+01 3,52E-01 0 3,03E-02 1,28E-01 3,91E-03 -1,58E+00
SM kg 1,27E-02 0,00E+00 0 0,00E+00 0,00E+00 0,00E+00 0,00E+00
RSF MJ 0,00E+00 0,00E+00 0 0,00E+00 0,00E+00 0,00E+00 -5,88E-05
NRSF MJ 0,00E+00 0,00E+00 0 0,00E+00 0,00E+00 0,00E+00 0,00E+00
W m3 1,83E-02 6,59E-05 0 5,73E-06 4,28E-03 4,03E-06 -4,83E-03
RPEE Renewable primary energy resources used as energy carrier; RPEM Renewable primary energy resources used as raw materials; TPE Total use of renewable
primary energy resources; NRPE Non renewable primary energy resources used as energy carrier; NRPM Non renewable primary energy resources used as
materials; TRPE Total use of non renewable primary energy resources; SM Use of secondary materials; RSF Use of renewable secondary fuels; NRSF Use of non
renewable secondary fuels; W Use of net fresh water
"Reading example: 9,0 E-03 = 9,0*10-3 = 0,009"
*INA Indicator Not Assessed
End of life - Waste
Parameter Unit A1-A3 A4 C1 C2 C3 C4 D
HW kg 1,01E-03 2,05E-07 0 1,78E-08 4,54E-07 4,31E-09 -2,04E-06
NHW kg 4,18E+00 1,85E-02 0 1,62E-03 7,45E-03 1,21E-02 -1,27E+00
RW kg 2,43E-05 2,41E-06 0 2,08E-07 6,52E-07 2,37E-08 -6,53E-06
HW Hazardous waste disposed; NHW Non hazardous waste disposed; RW Radioactive waste disposed
"Reading example: 9,0 E-03 = 9,0*10-3 = 0,009"
*INA Indicator Not Assessed
End of life - Output flow
Parameter Unit A1-A3 A4 C1 C2 C3 C4 D
CR kg 0,00E+00 0,00E+00 0 0,00E+00 0,00E+00 0,00E+00 0,00E+00
MR kg 1,17E-03 0,00E+00 0 0,00E+00 5,73E-02 0,00E+00 0,00E+00
MER kg 3,13E-05 0,00E+00 0 0,00E+00 8,10E-02 0,00E+00 0,00E+00
EEE MJ 7,17E-05 0,00E+00 0 0,00E+00 1,82E-01 0,00E+00 0,00E+00
ETE MJ 1,40E-04 0,00E+00 0 0,00E+00 1,25E+00 0,00E+00 0,00E+00
CR Components for reuse; MR Materials for recycling; MER Materials for energy recovery; EEE Exported electric energy; ETE Exported thermal energy
"Reading example: 9,0 E-03 = 9,0*10-3 = 0,009"
*INA Indicator Not Assessed
NEPD-3360-1989-EN 3G2,5 PFXP-LX-ER WHITE (ver2-040422) 7 / 8
Additional Norwegian requirements
Greenhouse gas emissions from the use of electricity in the manufacturing phase
National production mix from import, low voltage (production of transmission lines, in addition to direct emissions and losses in grid) of applied electricity for
the manufacturing process (A3).
Electricity mix Data source Amount Unit
Danish wind power - Renewable electricity with Guarantee of Origin from
ecoinvent 3.6 15,08 g CO2-ekv/kWh
EAC (kWh)
Dangerous substances
The product contains no substances given by the REACH Candidate list or the Norwegian priority list.
Indoor environment
Bibliography
ISO 14025:2010 Environmental labels and declarations - Type III environmental declarations - Principles and procedures.
ISO 14044:2006 Environmental management - Life cycle assessment - Requirements and guidelines.
EN 15804:2012+A1:2013 Environmental product declaration - Core rules for the product category of construction products.
ISO 21930:2017 Sustainability in buildings and civil engineering works - Core rules for environmental product declarations of construction products.
ecoinvent v3, Allocation, cut-off by classification, Swiss Centre of Life Cycle Inventories.
Iversen et al., (2018) eEPD v3- Background information for EPD generator system. LCA.no report 04.18. Iversen et al., (2020) EPD generator for Elektroskandia and Prysmian Group
- Background information and LCA data, LCA.no report 01.20
NPCR Part A: Construction products and services. Ver. 1.04.2017 EPD-Norge. NPCR 27 Part B for electrical cables and wires or NPCR 28 Part B for cable pipes Ver. 1.02.2020 EPD-
Norge.
Program operator and publisher Phone: +47 23 08 80 00
The Norwegian EPD Foundation e-mail: post@epd-norge.no
Post Box 5250 Majorstuen, 0303 Oslo,Norway web: www.epd-norge.no
Owner of the declaration Phone: +47 97 66 22 12
Elektroskandia Norge AS e-mail: pkr@elektroskandia.no
Postboks 143 1403 Langhus web: elektroskandia.no
Author of the Life Cycle Assessment Phone: +47 916 50 916
LCA.no AS e-mail: post@lca.no
Dokka 1C 1671 Kråkerøy web: www.lca.no
Developer of EPD generator Phone: +47 916 50 916
LCA.no AS e-mail: post@lca.no
Dokka 1C,1671 Kråkerøy web: www.lca.no
NEPD-3360-1989-EN 3G2,5 PFXP-LX-ER WHITE (ver2-040422) 8 / 8
