Environmental product declaration
in accordance with ISO 14025 and EN 15804+A2
SafeRing/SafePlus 12/24 kV type CCF Arc Classified
Owner of the declaration: Program operator:
ABB Electrification Norway AS The Norwegian EPD Foundation
Product: Declaration number:
SafeRing/SafePlus 12/24 kV type CCF Arc Classified
NEPD-5137-4465-EN
Declared unit:
1 pcs Registration number:
This declaration is based on Product Category Rules: NEPD-5137-4465-EN
EN 15804:2012+A2:2019 serves as core PCRs. EN
Issue date: 11.10.2023
50693:2019
The Norwegian EPD Foundation
PCR EPDItaly015 - Electronic and electrical products and Valid to: 11.10.2028
systems - Switchboards
EPD Software:
LCA.no EPD generator ID: 71873
1 / 12
General information
Product Owner of the declaration:
SafeRing/SafePlus 12/24 kV type CCF Arc Classified ABB Electrification Norway AS
Contact person: Magnus Nystad-Hansen
Phone: +47 35 58 20 21
e-mail: magnus.nystad-hansen@no.abb.com
Program operator: Manufacturer:
Post Box 5250 Majorstuen, 0303 Oslo, Norway ABB Electrification Norway AS
The Norwegian EPD Foundation Amtm. Aallsgt. 73
Phone: +47 23 08 80 00 3716 Skien, Norway
web: post@epd-norge.no
Declaration number: NEPD-5137-4465-EN Place of production:
ABB Electrification Norway AS, Skien
Amtm. Aallsgate 73
3701 Skien, Norway
This declaration is based on Product Category Rules: Management system:
EN 15804:2012+A2:2019 serves as core PCRs. EN 50693:2019 ISO 9001, ISO 14001
PCR EPDItaly015 - Electronic and electrical products and systems -
Switchboards
Statement of liability: Organisation no:
The owner of the declaration shall be liable for the underlying 921 186 037
information and evidence. EPD Norway shall not be liable with respect
to manufacturer information, life cycle assessment data and
evidences.​
Declared unit: Issue date: 11.10.2023
1 pcs SafeRing/SafePlus 12/24 kV type CCF Arc Classified
Declared unit with option: Valid to: 11.10.2028
A1-A3,A4,A5,B1,B6,C1,C2,C3,C4,D
Year of study:
2022
Functional Unit Comparability:
Declared unit for 1 SafeRing/SafePlus 12/ 24 kV type CCF Arc EPDs from other programmes than EPD Norway may not be
Classified, including packaging with optional modules B1, B6, C1-C4 comparable.
and D.
General information on verification of EPD from EPD tools: Development and verification of EPD:
Independent verification of data, other environmental information The declaration is created using EPD tool lca.tools ver EPD2022.03,
and the declaration according to ISO 14025:2010, § 8.1.3 and § 8.1.4. developed by LCA.no. The EPD tool is integrated in the company's
Verification of each EPD is made according to EPD-Norway’s management system, and has been approved by EPD Norway.
guidelines for verification and approval requiring that tools are i
integrated into the company's environmental management system, ii Developer of EPD: Magnus Nystad-Hansen
the procedures for use of the EPD tool are approved by EPD-Norway,
Reviewer of company-specific input data and EPD: Magnus Bjerkely
and iii the process is reviewed annually by an independent third
party verifier. See Appendix G of EPD-Norway's General Programme
Instructions for further information on EPD tools
Verification of EPD tool: Approved:
Independent third party verification of the EPD tool, background data
and test-EPD in accordance with EPDNorway's procedures and
guidelines for verification and approval of EPD tools.
Third party verifier:
Jane Anderson, Construction LCA Håkon Hauan, CEO EPD-Norge
(no signature required
2 / 12
Product
Product description:
ABB SafeRing/SafePlus Switchgear is a medium voltage gas insulated ring main unit for secondary distribution. The main function of the
switchgears is to “establish and cut off the supply of a downstream installation from an electrical and/or mechanical control and to protect people
and premises at risk of fire or explosion against insulation defects”. SafeRing/SafePlus can be supplied in a number of different configurations
suitable for most switching applications in 12/24 kV distribution networks.
SafeRing/SafePlus 12 / 24 kV type CCVF Arc Classified switchgear consist of two load-break switch units (C-module) plus one switch-fuse
combination unit (F-module).
The manufacturer proclaims a minimum product service life of 30 years but the calculations are based on 20 years as the PCR dictates.
The functional unit of this study is described as 1 piece of SafeRing/SafePlus 12 / 24 kV type CCF Arc Classified including heat loss during a 20
year product lifetime. The functional unit is IAC classified.
Product specification
Materials kg %
Plastics 14,70 4,42
Epoxy resin insulator, Al2O3 18,68 5,62
Metal 299,11 89,96
Total 332,48
Packaging kg %
Packaging - Pallet 34,49 100,00
Total incl. packaging 366,97
Technical data:
Parameter Amount
Rated voltage: 12 / 24 kV
Rated frequency: 50 Hz
Rated nominal current: 630 A
Rated power frequency withstand voltage: 28 / 50 kV
Rated lightning impulse withstand voltage: 95 / 125 kV
Rated short-time withstand current: 25 / 21 kA
Rated duration of short-circuit: 3 s
Rated peak withstand current: 62.5 / 52.5 kA
Insulating medium: SF6
Rated filling pressure at 20 degree Celsius: 0.14 MPa (absolute)
Internal arc classification: IAC AFL 20 kA, 1.0 s
Market:
Norway
Reference service life, product
20
Reference service life, building
N/A
LCA: Calculation rules
Declared unit:
1 pcs SafeRing/SafePlus 12/24 kV type CCF Arc Classified
Cut-off criteria:
All major raw materials and all the essential energy is included. The production processes for raw materials and energy flows with very small
amounts (less than 2%) might not be included. These cut-off criteria do not​ apply for hazardous materials and substances.
Allocation:
The allocation is made in accordance with the provisions of EN 15804. Incoming energy and water and waste production in-house is allocated
equally among all products through time allocation. Effects of primary production of recycled materials is allocated to the main product in which
the material was used. The recycling process and transportation of the material is allocated to this analysis.
Data quality:
3 / 12
Specific data for the product composition are provided by the manufacturer. They represent the production of the declared product and were
collected for EPD development in the year of study. Background data is based on EPDs according to EN 15804, Norsus, ecoinvent and other LCA
databases. The data quality of the raw materials in A1 is presented in the table below.
Materials Source Data quality Year
Plastics CEPE 3.0 Database 2022
Epoxy resin insulator, Al2O3 ecoinvent 3.6 Database 2019
Metal ecoinvent 3.6 Database 2019
Packaging - Pallet ecoinvent 3.6 Database 2019
Plastics ecoinvent 3.6 Database 2019
Plastics Industry data 2.0 Database 2019
4 / 12
System boundaries (X=included, MND=module not declared, MNR=module not relevant)
Construction Beyond the system
Product stage Use stage End of life stage
installation stage boundaries
A1 A2 A3 A4 A5 B1 B2 B3 B4 B5 B6 B7 C1 C2 C3 C4 D
X X X X X X MND MND MND MND X MND X X X X X
System boundary:
Additional technical information:
No additional technical information has been provided in this EPD.
waR slairetam tropsnarT gnirutcafunaM tropsnarT ylbmessA e​sU ecnanetniaM riapeR tnemecalpeR tnemhsibrufeR lanoitarepO ygrene esu lanoitarepO esu retaw -eD noitcurtsnoc noitilomed tropsnarT etsaW gnissecorp lasopsiD -yrevoceR-esueR laitnetop-gnilcyceR
5 / 12
LCA: Scenarios and additional technical information
The following information describe the scenarios in the different modules of the EPD.
The product is assumed to be transported to an installation site in Norway in module A4.
The impact of installing the unit in A5 is assumed to be very low and is set as 0. B1 includes 0.1 % yearly leakage of insulating medium during
reference service life, based confirmation certificate for the product.
B6 includes electricity lost through heat loss during reference service life in accordance with the PCR. Heat loss during service is based on the
resistance on the electrical circuit and 50 % loading relative to nominal current. This analysis is based on Norwegian electricity mix in B6.
The impact of removing the unit from it's place of usage (C1) to transport is assumed to be very low and is set as 0.
In C2 the switchgear is assumed to be transported to a waste treatment facility in Norway.
The waste treatment company has a process for collection and incineration of all remaining insulating medium in the unit. There is no leakage of
insulating medium during the disassembly.
End-of-life treatment scenarios for the product in modules C3 and C4 are based on the default values given in EN 50963 Annex G, Table G.4
Capacity utilisation Value
Transport from production place to user (A4) Distance (km) Fuel/Energy Consumption Unit
(incl. return) % (Liter/tonn)
Truck, 16-32 tonnes, EURO 5 - RER 36,7 % 132 0,044 l/tkm 5,81
Assembly (A5) Unit Value
Waste, packaging, Pallet, EUR wooden pallet,
kg 34,49
average treatment (kg)
Use (B1) Unit Value
SF6 leakage (kg) - GLO kg/DU 0,07
Operational energy (B6) and water
Unit Value
consumption (B7)
Electricity, Norway, medium voltage (kWh) kWh/DU 12302,11
Capacity utilisation Value
Transport to waste processing (C2) Distance (km) Fuel/Energy Consumption Unit
(incl. return) % (Liter/tonn)
Truck, 16-32 tonnes, EURO 5 - RER 36,7 % 132 0,044 l/tkm 5,81
Waste processing (C3) Unit Value
Aluminium to recycling (kg) kg 6,10
Copper to recycling (kg) kg 21,90
Other non-ferrous metals to recycling (kg) kg 3,90
Steel to recycling (kg) kg 197,92
Waste treatment per kg Plastics mixture,
kg 7,42
incineration (kg)
Waste, Hazardous, incineration (kg) kg 20,44
Disposal (C4) Unit Value
Disposal, landfilling of aluminium (kg) kg 2,61
Disposal, landfilling of copper (kg) kg 14,60
Disposal, landfilling of other non-ferrous
kg 2,60
metals(kg)
Disposal, landfilling of steel (kg) kg 49,48
Landfilling of ashes from incineration of Plastics
kg 0,23
mixture (kg)
Landfilling of mixed plastics (kg) kg 5,51
Benefits and loads beyond the system
Unit Value
boundaries (D)
Substitution of electricity, in Norway (MJ) MJ 40,70
Substitution of primary aluminium with net scrap
kg 6,10
(kg)|
Substitution of primary copper with net scrap (kg) kg 14,45
Substitution of primary other non-ferrous metals
kg 3,90
with net scrap (kg)
Substitution of primary steel with net scrap (kg) kg 141,73
Substitution of thermal energy, district heating, in
MJ 383,31
Norway (MJ)
6 / 12
LCA: Results
The LCA results are presented below for the declared unit defined on page 2 of the EPD document.
Environmental impact
Indicator Unit A1-A3 A4 A5 B1 B6 C1 C2 C3 C4 D
GWP-total
kg CO2 -
2,05E+03 8,08E+00 5,32E+01 1,81E+03 2,61E+02 0 8,08E+00 6,71E+01 5,46E+01 -2,53E+02
eq
GWP-fossil
kg CO2 -
2,10E+03 8,07E+00 9,28E-01 1,81E+03 2,52E+02 0 8,07E+00 6,71E+01 4,10E+00 -2,51E+02
eq
GWP-biogenic
kg CO2 -
-5,12E+01 3,29E-03 5,23E+01 0,00E+00 7,47E+00 0 3,29E-03 3,82E-04 5,05E+01 -5,05E-01
eq
GWP-luluc
kg CO2 -
2,11E+00 2,82E-03 2,38E-04 0,00E+00 1,11E+00 0 2,82E-03 9,84E-03 3,18E-04 -1,21E+00
eq
kg
ODP CFC11 - 1,36E-04 1,84E-06 1,48E-07 0,00E+00 1,68E-05 0 1,84E-06 5,85E-06 2,50E-07 -1,62E-01
eq
mol H+
AP 3,44E+01 3,30E-02 7,46E-03 0,00E+00 1,01E+00 0 3,30E-02 7,61E-02 9,47E-03 -6,98E+00
-eq
EP-FreshWater kg P -eq 6,51E-01 6,34E-05 1,11E-05 0,00E+00 1,07E-02 0 6,34E-05 1,08E-03 3,36E-04 -5,12E-02
EP-Marine kg N -eq 3,42E+00 9,79E-03 3,20E-03 0,00E+00 1,76E-01 0 9,79E-03 1,62E-02 8,50E-02 -4,55E-01
mol N -
EP-Terrestial 4,20E+01 1,08E-01 3,43E-02 0,00E+00 2,20E+00 0 1,08E-01 1,79E-01 2,92E-02 -5,95E+00
eq
kg
POCP NMVOC 1,26E+01 3,31E-02 8,82E-03 0,00E+00 5,78E-01 0 3,31E-02 4,81E-02 2,25E-02 -2,00E+00
-eq
ADP- kg Sb -
2,71E-01 2,19E-04 1,51E-05 0,00E+00 6,32E-03 0 2,19E-04 1,04E-04 7,33E-06 -3,52E-02
minerals&metals1 eq
ADP-fossil1 MJ 2,50E+04 1,22E+02 1,09E+01 0,00E+00 3,51E+03 0 1,22E+02 2,36E+02 2,01E+01 -2,38E+03
WDP1 m3 1,66E+04 1,16E+02 1,68E+01 0,00E+00 6,49E+05 0 1,16E+02 2,40E+01 5,02E+02 -2,15E+04
GWP-total = Global Warming Potential total; GWP-fossil = Global Warming Potential fossil fuels; GWP-biogenic = Global Warming Potential biogenic; GWP-luluc =
Global Warming Potential land use and land use change; ODP = Depletion potential of the stratospheric ozone layer; AP = Acidification potential, Accumulated
Exceedance; EP-freshwater = Eutrophication potential, fraction of nutrients reaching freshwater end compartment: EP-marine = Eutrophication potential, fraction of
nutrients reaching marine end compartment; EP-terrestrial = Eutrophication potential, Accumulated Exceedance; POCP = Formation potential of tropospheric ozone;
ADP-minerals&metals = Abiotic depletion potential for non-fossil resources; ADP-fossil = Abiotic depletion for fossil resources potential; WDP = Water (user)
deprivation potential, deprivation-weighted water consumption
"Reading example: 9,0 E-03 = 9,0*10-3 = 0,009"
*INA Indicator Not Assessed
1. The results of this environmental impact indicator shall be used with care as the uncertainties on these results are high or as there is limited experienced with the
indicator
3. Eutrophication aquatic freshwater shall be in kg P-eq., there is a typo in EN 15804:2012+A2:2019 regarding this unit. Eutrophication calculated as PO4-eq is presented
on page 11
Remarks to environmental impacts
7 / 12
Additional environmental impact indicators
Indicator Unit A1-A3 A4 A5 B1 B6 C1 C2 C3 C4 D
PM Disease incidence 1,93E-04 5,81E-07 9,12E-08 0,00E+00 9,41E-06 0 5,81E-07 6,83E-07 1,25E-07 -2,98E-05
IRP2 kgBq U235 -eq 9,47E+01 5,32E-01 3,95E-02 0,00E+00 6,70E+01 0 5,32E-01 1,01E+00 1,36E-01 -3,03E+00
ETP-fw1 CTUe 3,46E+05 8,97E+01 1,24E+01 5,71E-03 6,12E+03 0 8,97E+01 9,96E+02 1,82E+03 -6,33E+04
HTP-c1 CTUh 1,65E-05 0,00E+00 1,38E-09 1,00E-12 3,32E-07 0 0,00E+00 3,21E-08 2,51E-09 -1,66E-06
HTP-nc1 CTUh 3,65E-04 9,69E-08 6,63E-08 1,00E-12 6,30E-06 0 9,69E-08 3,81E-07 3,16E-08 -4,95E-05
SQP1 dimensionless 1,86E+04 8,39E+01 6,11E+00 0,00E+00 1,65E+03 0 8,39E+01 5,06E+01 6,49E+01 -9,97E+02
PM = Particulate Matter emissions; IRP = Ionizing radiation – human health; ETP-fw = Eco toxicity – freshwater; HTP-c = Human toxicity – cancer effects; HTP-nc =
Human toxicity – non cancer effects; SQP = Potential Soil Quality Index (dimensionless)
"Reading example: 9,0 E-03 = 9,0*10-3 = 0,009"
*INA Indicator Not Assessed
1. The results of this environmental impact indicator shall be used with care as the uncertainties on these results are high or as there is limited experienced with the
indicator
2. This impact category deals mainly with the eventual impact of low dose ionizing radiation on human health of the nuclear fuel cycle. It does not consider effects due
to possible nuclear accidents, occupational exposure nor due to radioactive waste disposal in underground facilities. Potential ionizing radiation from the soil, from
radon and from some construction materials is also not measured by this indicator.
8 / 12
Resource use
Indicator Unit A1-A3 A4 A5 B1 B6 C1 C2 C3 C4 D
PERE MJ 4,41E+03 1,72E+00 2,24E-01 0,00E+00 4,81E+04 0 1,72E+00 9,78E+00 2,48E+00 -6,97E+02
PERM MJ 4,79E+02 0,00E+00 -4,79E+02 0,00E+00 0,00E+00 0 0,00E+00 0,00E+00 0,00E+00 0,00E+00
PERT MJ 4,89E+03 1,72E+00 -4,79E+02 0,00E+00 4,81E+04 0 1,72E+00 9,78E+00 2,48E+00 -6,97E+02
PENRE MJ 2,50E+04 1,22E+02 1,09E+01 0,00E+00 3,51E+03 0 1,22E+02 2,36E+02 2,01E+01 -2,38E+03
PENRM MJ 3,71E+02 0,00E+00 0,00E+00 0,00E+00 0,00E+00 0 0,00E+00 0,00E+00 0,00E+00 0,00E+00
PENRT MJ 2,51E+04 1,22E+02 1,09E+01 0,00E+00 3,51E+03 0 1,22E+02 2,36E+02 2,01E+01 -2,38E+03
SM kg 6,37E+01 0,00E+00 0,00E+00 0,00E+00 0,00E+00 0 0,00E+00 0,00E+00 1,37E-02 1,01E+01
RSF MJ 1,28E+01 6,15E-02 6,54E-03 0,00E+00 3,77E+01 0 6,15E-02 2,89E-03 5,14E-02 6,60E+00
NRSF MJ 1,12E+02 2,20E-01 7,45E-02 0,00E+00 9,91E+01 0 2,20E-01 0,00E+00 2,30E-02 1,59E+02
FW m3 2,45E+01 1,28E-02 7,94E-03 0,00E+00 3,60E+02 0 1,28E-02 1,94E-01 2,72E-02 -2,91E+00
PERE = Use of renewable primary energy excluding renewable primary energy resources used as raw materials; PERM = Use of renewable primary energy resources used
as raw materials; PERT = Total use of renewable primary energy resources; PENRE = Use of non renewable primary energy excluding non-renewable primary energy
resources used as raw materials; PENRM = Use of non renewable primary energy resources used as raw materials; PENRT = Total use of non renewable primary energy
resources; SM = Use of secondary materials; RSF = Use of renewable secondary fuels; NRSF = Use of non-renewable secondary fuels; FW = Net use of fresh water
"Reading example: 9,0 E-03 = 9,0*10-3 = 0,009"
*INA Indicator Not Assessed
9 / 12
End of life - Waste
Indicator Unit A1-A3 A4 A5 B1 B6 C1 C2 C3 C4 D
HWD kg 7,15E+00 6,21E-03 0,00E+00 0,00E+00 6,63E-01 0 6,21E-03 8,38E-04 1,56E-01 -9,98E-01
NHWD kg 5,83E+03 5,82E+00 3,45E+01 0,00E+00 2,77E+02 0 5,82E+00 1,11E+01 7,49E+01 -9,87E+01
RWD kg 6,38E-02 8,30E-04 0,00E+00 0,00E+00 3,28E-02 0 8,30E-04 1,39E-03 1,45E-04 -2,90E-03
HWD = Hazardous waste disposed; NHWD = Non-hazardous waste disposed; RWD = Radioactive waste disposed
"Reading example: 9,0 E-03 = 9,0*10-3 = 0,009"
*INA Indicator Not Assessed
End of life - Output flow
Indicator Unit A1-A3 A4 A5 B1 B6 C1 C2 C3 C4 D
CRU kg 0,00E+00 0,00E+00 0,00E+00 0,00E+00 0,00E+00 0 0,00E+00 0,00E+00 0,00E+00 0,00E+00
MFR kg 0,00E+00 0,00E+00 8,09E-04 0,00E+00 0,00E+00 0 0,00E+00 2,30E+02 5,19E-04 -3,95E-01
MER kg 3,67E-01 0,00E+00 3,42E+01 0,00E+00 0,00E+00 0 0,00E+00 2,79E+01 3,42E-04 -5,21E-02
EEE MJ 1,24E+00 0,00E+00 2,38E+01 0,00E+00 0,00E+00 0 0,00E+00 3,92E+01 3,72E-03 -1,28E-01
EET MJ 8,50E+00 0,00E+00 3,60E+02 0,00E+00 0,00E+00 0 0,00E+00 3,64E+02 5,62E-02 -1,93E+00
CRU = Components for re-use; MFR = Materials for recycling; MER = Materials for energy recovery; EEE = Exported energy electrical; EET = Exported energy thermal
"Reading example: 9,0 E-03 = 9,0*10-3 = 0,009"
*INA Indicator Not Assessed
Biogenic Carbon Content
Indicator Unit At the factory gate
Biogenic carbon content in product kg C 0,00E+00
Biogenic carbon content in accompanying packaging kg C 1,43E+01
Note: 1 kg biogenic carbon is equivalent to 44/12 kg CO2
10 / 12
Additional requirements
Greenhouse gas emissions from the use of electricity in the manufacturing phase
National production mix from import, low voltage (production of transmission lines, in addition to direct emissions and losses in grid) of applied
electricity for the manufacturing process (A3).
Electricity mix Data source Amount Unit
Electricity, Norway, medium voltage (kWh) ecoinvent 3.6 21,18 g CO2-eq/kWh
Dangerous substances
The product contains no substances given by the REACH Candidate list.
Indoor environment
Additional Environmental Information
Additional environmental impact indicators required in NPCR Part A for construction products
Indicator Unit A1-A3 A4 A5 B1 B6 C1 C2 C3 C4 D
GWPIOBC kg CO2 -eq 2,09E+03 8,08E+00 0,00E+00 1,58E+03 2,93E+02 0 8,08E+00 6,69E+01 6,43E-02 -3,12E+02
GWP-IOBC: Global warming potential calculated according to the principle of instantaneous oxidation. In order to increase the transparency of biogenic carbon​
contribution to climate impact, the indicator GWP-IOBC is required as it declares climate impacts calculated according to the principle of instantaneous oxidation.​
GWP-IOBC is also referred to as GWP-GHG in context to Swedish public procurement legislation.
11 / 12
Bibliography
ISO 14025:2010 Environmental labels and declarations - Type III environmental declarations - Principles and procedures.
ISO 14044:2006 Environmental management - Life cycle assessment - Requirements and guidelines.
EN 15804:2012+A2:2019 Environmental product declaration - Core rules for the product category of construction products.
ecoinvent v3, Allocation, cut-off by classification, Swiss Centre of Life Cycle Inventories.
Iversen et al., (2021) eEPD v2021.09 Background information for EPD generator tool system verification, LCA.no Report number: 07.21.
Vold et al (2021) EPD generator for ABB, Background information for customer application and LCA data, LCA.no Report number: 09.21
EN 50693:2019 Product category rules for life cycle assessment of electronic and electrical products and systems.
PCR EPDItaly015 Electronic and electrical products and systems, Switchboards.
Program operator and publisher Phone: +47 23 08 80 00
The Norwegian EPD Foundation e-mail: post@epd-norge.no
Post Box 5250 Majorstuen, 0303 Oslo, Norway web: www.epd-norge.no
Owner of the declaration: Phone: +47 35 58 20 21
magnus.nystad-
ABB Electrification Norway AS e-mail:
hansen@no.abb.com
Amtm. Aallsgt. 73, 3716 Skien web: https://new.abb.com/
Author of the Life Cycle Assessment Phone: +47 69 35 11 00
Norsus AS e-mail: post@norsus.no
Stadion 4, 1671 web: www.norsus.no
Developer of EPD generator Phone: +47 916 50 916
LCA.no AS e-mail: post@lca.no
Dokka 6B,1671 Kråkerøy web: www.lca.no
ECO Platform web: www.eco-platform.org
ECO Portal web: ECO Portal
12 / 12
