ver1 2015
ENVIRONMENTAL PRODUCT DECLARATION
in accordance with ISO 14025, ISO 21930 and EN 15804
Owner of the declaration: JSC Svenheim
Program operator: The Norwegian EPD Foundation
Publisher: The Norwegian EPD Foundation
Declaration number: NEPD-2648-1355-EN
Registration number: NEPD-2648-1355-EN
ECO Platform reference number: -
Issue date: 01.02.2021
Valid to: 01.02.2026
Optima conference table 6000x1200 grey HPL
JSC Svenheim
www.epd-norge.no
NEPD-2648-1355-EN Optima conference table 6000x1200 grey HPL 1 / 8
General information
Product: Owner of the declaration:
Optima conference table 6000x1200 grey HPL
JSC Svenheim
Contact person: Karolina Klimaite
Phone: +370 657 52044
e-mail: info@svenheim.lt
Program operator: Manufacturer:
JSC Svenheim
The Norwegian EPD Foundation
Naujoji str.132 , LT-62175 Alytus
Pb. 5250 Majorstuen, 0303 Oslo
Lithuania
Phone: +47 23 08 80 00
e-mail: post@epd-norge.no
Declaration number: Place of production:
JSC Svenheim
NEPD-2648-1355-EN Naujoji str.132 , LT-62175 Alytus
Lithuania
ECO Platform reference number: Management system:
ISO 14001, Certificate No. 81858-2010-AE-LUT-FINAS ISO 9001, Certificate No.
81860-2010-AQ-LTU-FINAS Accredited unit: DNV Certification OY/AB, Finland
This declaration is based on Product Category Rules: Organisation no:
LT100004040014
CEN Standard EN 15804:2012+A1:2013 serves as core PCR
Statement of liability: Issue date: 01.02.2021
The owner of the declaration shall be liable for the underlying information and
evidence. EPD Norway shall not be liable with respect to manufacturer Valid to: 01.02.2026
information, life cycle assessment data and evidences.
Declared unit: Year of study:
1 Pcs Optima conference table 6000x1200 grey HPL
Declared unit with option: Comparability:
A1,A2,A3,A4,C1,C2,C3,C4,D EPDs from programmes other than the Norwegian EPD Foundation may not be
comparable
Functional unit: Development and verification of EPD:
The declaration has been developed and verified using EPD tool lca.tools
ver EPD2020.11, developed by LCA.no AS. The EPD tool is integrated into
the company's environmental management system, and has been
approved by EPD-Norway
General information on verification of EPD from EPD tools:
Independent verification of data, other environmental information and Developer of EPD:
the declaration according to ISO 14025:2010, § 8.1.3 and § 8.1.4. Individual
third party verification of each EPD is not required when the EPD tool is i) Karolina Klimaite
integrated into the company's environmental management system, ii) the
procedures for use of the EPD tool are approved by EPDNorway, and iii) Reviewer of company-specific input data and EPD:
the proccess is reviewed annualy. See Appendix G of EPD-Norway's
General Programme Instructions for further information on EPD tools. Linas Vosylius
Verification of EPD tool: Approved:
Independent third party verification of the EPD tool, background data
Sign
and test-EPD in accordance with EPDNorway's procedures and guidelines
for verification and approval of EPD tools.
Erik Svanes, Norsus AS
(no signature required) Håkon Hauan, CEO EPD-Norge
Key environmental indicators Unit Cradle to gate A1 - A3
Global warming kg CO2 eqv 388,87
Total energy use MJ 10385,36
Amount of recycled materials % 2,57
NEPD-2648-1355-EN Optima conference table 6000x1200 grey HPL 2 / 8
Product
Market: Technical data:
Europe Total weight 208,89kg (with packaging)
Product description: Reference service life, product
Meeting table Optima, rect. shape 4000*1200*26, grey HPL with fixed
15 years
round column 735mm, Astro T-foot
Reference service life, building
Product specification
Optima conference table has core material in 25 mm MDF, with surface
selection of veneer, linoleum, HT laminate, Fenix black matt HT
laminate as standard. The edge is profiled 10 mm straight with 40
degrees chamfer or as straight edge with radius 2mm. Veneered surface
has 5 coats of UV lacquer, which makes the surface very durable and
strong. Legs has fixed or electric column, T-foot, X-foot or disk-foot.
Surfaces in gray, white, black or chrome.
Recycled share in Recycled share in
Materials kg %
material (kg) material (%)
Printed paper 0,95 0,34 0,00 0,00
Metal - Steel 31,51 11,32 6,30 20,00
Wood - Medium Density Fibreboard (MDF) 236,16 84,85 0,00 0,00
Plastic - Acrylonitrile butadiene styrene (ABS) 0,62 0,22 0,00 0,00
Plastic - Polypropylene (PP) 0,00 0,00 0,00 0,00
Wood - Solid beech/birch 0,05 0,02 0,00 0,00
Glue for wood 2,91 1,05 0,00 0,00
High pressure laminate - HPL thin 6,14 2,21 0,02 0,39
Recycled share in Recycled share in
Packaging kg
material (kg) material (%)
Packaging - Cardboard 0,41 0,31 76,30
Packaging - Cardboard 2,00 1,53 76,30
LCA: Calculation rules
Declared unit: Allocation:
The allocation is made in accordance with the provisions of EN 15804. Effects
1 Pcs Optima conference table 6000x1200 grey HPL
of primary production of recycled materials is allocated to the main product
Cut-off criteria: in which the material was used. The recycling process and transportation of
the material is allocated to this analysis.
All major raw materials and all the essential energy is included. The
production processes for raw materials and energy flows with very small
amounts (less than 1%) are not included. These cut-off criteria do not
apply for hazardous materials and substances.
Data quality:
Specific data for the product composition are provided by the manufacturer. They represent the production of the declared product and were collected for
EPD development in the year of study. Background data is based on registered EPDs according to EN 15804, Ostfold Research databases, ecoinvent and other
LCA databases. The data quality of the raw materials in A1 is presented in the table below.
Materials Source Data quality Year
Plastic - Polypropylene (PP) ecoinvent 3.4 Database 2015
Plastic - Acrylonitrile butadiene styrene (ABS) PlasticsEurope EPD 2015
Metal - Steel ecoinvent 3.3 Database 2016
Glue for wood ecoinvent 3.4 Database 2017
Metal - Steel ecoinvent 3.4 Database 2017
Packaging - Cardboard ecoinvent 3.4 Database 2017
Printed paper ecoinvent 3.4 Database 2017
Wood - Medium Density Fibreboard (MDF) ecoinvent 3.4 Database 2017
Wood - Solid beech/birch ecoinvent 3.4 Database 2017
High pressure laminate - HPL thin EPD-ICL-20170155-CBE1-EN EPD, IBU 2017
NEPD-2648-1355-EN Optima conference table 6000x1200 grey HPL 3 / 8
System boundary:
Additional technical information:
Transportation to an average customer in Norway is 1606 km (A4: average European lorry > 32 tonnes) (Transport, freight, by lorry (>32t): 1426 km and by sea
transport: 180 km).
The electricity consumed is assumed to be from East pool mix in the East European countries. European mix and energy mix in Lithuania is based on data
from the World bank (Based on data 2011).
Electricity mix: 0,053 kg CO2 eqv/MJ (East Europe mix).
NEPD-2648-1355-EN Optima conference table 6000x1200 grey HPL 4 / 8
The following information describe the scenarios in the different modules of the EPD.
The following information describe the scenarios in the different modules of the EPD.
In the end of life stage, the transport distance for waste to waste processing is 72 km (C1). The reuse, recovery and recycling stage is beyond the system
boundaries (D). It is assumed that the solution is dismantled and the materials recycled. In the table below Norwegian treatment of industrial waste is
calculated. This calculation includes only CO2 emissions (GWP) in the Cmodules. The transport distance to reuse, recovery or recycling varies for each material,
but the average distance is 373 km. The vehicles used and associated data are described in detail in [5].
Transport from production place to user (A4)
Capacity utilisation Fuel/Energy
Type Type of vehicle Distance km Unit Value (l/t)
(incl. return) % consumption
Truck 55,0 % Truck, over 32 tonnes, EURO 6 1426 0,022606 l/tkm 32,24
Railway l/tkm
Boat 71,0 % Ship, Coastal Barge (250 - 3000t load) 490 0,011179 l/tkm 5,48
Other Transportation l/tkm
End of Life (C1, C3, C4)
. Unit Value
Hazardous waste disposed kg
Collected as mixed construction waste kg
Reuse kg
Recycling kg 238,5750
Energy recovery kg
To landfill kg
Transport to waste processing (C2)
Capacity utilisation Fuel/Energy
Type Type of vehicle Distance km Unit Value (l/t)
(incl. return) % consumption
Truck 38,8 % Truck, 16-32 tonnes, EURO 6 72 0,043626 l/tkm 3,14
Railway l/tkm
Boat l/tkm
Other Transportation l/tkm
¨
NEPD-2648-1355-EN Optima conference table 6000x1200 grey HPL 5 / 8
LCA: Results
The LCA results are presented below for the declared unit defined on page 2 of the EPD document.
System boundaries (X=included, MND=module not declared, MNR=module not relevant)
Construction Beyond the
Product stage installation User stage End of life stage . system
stage bondaries
A1 A2 A3 A4 A5 B1 B2 B3 B4 B5 B6 B7 C1 C2 C3 C4 . D
X X X X MND MND MND MND MND MND MND MND X X X X . X
Environmental impact
Parameter Unit A1 A2 A3 A4 C1 C2 C3 C4 D
GWP kg CO 2 -eq 3,11E+02 3,29E+01 4,46E+01 4,50E+01 0 3,65E+00 4,70E-06 0 0
ODP kg CFC11 -eq 2,94E-05 6,75E-06 2,34E-06 8,80E-06 0 6,87E-07 0,00E+00 0 0
POCP kg C 2H 4-eq 1,58E-01 5,15E-03 2,94E-02 7,09E-03 0 5,53E-04 7,25E-10 0 0
AP kg SO 2 -eq 1,51E+00 8,48E-02 2,35E-01 1,51E-01 0 8,58E-03 1,35E-08 0 0
EP kg PO 3- -eq 2,77E-01 1,17E-02 3,74E-02 2,48E-02 0 1,13E-03 2,17E-09 0 0
4
ADPM kg Sb -eq 1,84E-03 7,93E-05 6,91E-05 9,36E-05 0 1,13E-05 1,40E-11 0 0
ADPE MJ 4,57E+03 5,39E+02 4,94E+02 7,11E+02 0 5,51E+01 5,29E-05 0 0
GWP Global warming potential; ODP Depletion potential of the stratospheric ozone layer; POCP Formation potential of tropospheric photochemical oxidants;
AP Acidification potential of land and water; EP Eutrophication potential; ADPM Abiotic depletion potential for non fossil resources; ADPE Abiotic depletion
potential for fossil resources
Reading example: 9,0 E-03 = 9,0*10-3 = 0,009
*INA Indicator Not Assessed
waR slairetam tropsnarT gnirutcafunaM tropsnarT ylbmessA esU ecnanetniaM riapeR tnemecalpeR tnemhsibrufeR lanoitarepO ygrene esu lanoitarepO esu
retaw
-eD noitcurtsnoc noitilomed tropsnarT etsaW gnissecorp lasopsiD -yrevoceR-esueR -gnilcyceR laitnetop
NEPD-2648-1355-EN Optima conference table 6000x1200 grey HPL 6 / 8
Resource use
Parameter Unit A1 A2 A3 A4 C1 C2 C3 C4 D
RPEE MJ 3,51E+03 9,74E+00 5,33E+02 1,33E+01 0 8,14E-01 2,67E-06 0 0
RPEM MJ 2,28E+03 0,00E+00 0,00E+00 0,00E+00 0 0,00E+00 0,00E+00 0 0
TPE MJ 5,79E+03 9,74E+00 5,33E+02 1,33E+01 0 8,14E-01 2,67E-06 0 0
NRPE MJ 4,95E+03 5,56E+02 8,25E+02 7,34E+02 0 5,64E+01 5,80E-05 0 0
NRPM MJ 7,98E+01 0,00E+00 0,00E+00 0,00E+00 0 0,00E+00 0,00E+00 0 0
TRPE MJ 5,03E+03 5,56E+02 8,25E+02 7,34E+02 0 5,64E+01 5,80E-05 0 0
SM kg 8,16E+00 0,00E+00 0,00E+00 0,00E+00 0 0,00E+00 0,00E+00 0 0
RSF MJ 1,22E+00 0,00E+00 0,00E+00 0,00E+00 0 0,00E+00 0,00E+00 0 0
NRSF MJ 9,50E-01 0,00E+00 0,00E+00 0,00E+00 0 0,00E+00 0,00E+00 0 0
W m3 2,19E+00 1,31E-01 3,91E-01 1,74E-01 0 1,07E-02 1,33E-08 0 0
RPEE Renewable primary energy resources used as energy carrier; RPEM Renewable primary energy resources used as raw materials; TPE Total use of renewable
primary energy resources; NRPE Non renewable primary energy resources used as energy carrier; NRPM Non renewable primary energy resources used as
materials; TRPE Total use of non renewable primary energy resources; SM Use of secondary materials; RSF Use of renewable secondary fuels; NRSF Use of non
renewable secondary fuels; W Use of net fresh water
Reading example: 9,0 E-03 = 9,0*10-3 = 0,009
*INA Indicator Not Assessed
End of life - Waste
Parameter Unit A1 A2 A3 A4 C1 C2 C3 C4 D
HW kg 1,04E-02 2,97E-04 1,03E-03 4,17E-04 0 3,32E-05 4,80E-11 0 0
NHW kg 1,83E+02 5,01E+01 1,14E+01 5,94E+01 0 3,02E+00 3,49E-06 0 0
RW kg INA* INA* INA* INA* 0 INA* INA* 0 0
HW Hazardous waste disposed; NHW Non hazardous waste disposed; RW Radioactive waste disposed
Reading example: 9,0 E-03 = 9,0*10-3 = 0,009
*INA Indicator Not Assessed
End of life - Output flow
Parameter Unit A1 A2 A3 A4 C1 C2 C3 C4 D
CR kg 0,00E+00 0,00E+00 0,00E+00 0,00E+00 0 0,00E+00 0,00E+00 0 0
MR kg 0,00E+00 0,00E+00 0,00E+00 0,00E+00 0 0,00E+00 5,58E+04 0 0
MER kg 0,00E+00 0,00E+00 0,00E+00 0,00E+00 0 0,00E+00 8,06E-07 0 0
EEE MJ INA* INA* INA* INA* 0 INA* INA* 0 0
ETE MJ INA* INA* INA* INA* 0 INA* INA* 0 0
CR Components for reuse; MR Materials for recycling; MER Materials for energy recovery; EEE Exported electric energy; ETE Exported thermal energy
Reading example: 9,0 E-03 = 9,0*10-3 = 0,009
*INA Indicator Not Assessed
NEPD-2648-1355-EN Optima conference table 6000x1200 grey HPL 7 / 8
Additional Norwegian requirements
Greenhouse gas emissions from the use of electricity in the manufacturing phase
National production mix from import, low voltage (production of transmission lines, in addition to direct emissions and losses in grid) of applied electricity for the manufacturing
process (A3).
Dangerous substances
The product contains no substances given by the REACH Candidate list or the Norwegian priority list.
Indoor environment
Our furniture doesn't contain any constituent parts that affect indoor climate.
Additional environmental information
Bibliography
ISO 14025:2010 Environmental labels and declarations - Type III environmental declarations - Principles and procedures.
ISO 14044:2006 Environmental management - Life cycle assessment - Requirements and guidelines.
EN 15804:2012+A1:2013 Environmental product declaration - Core rules for the product category of construction products.
ISO 21930:2017 Sustainability in buildings and civil engineering works - Core rules for environmental product declarations of construction products.
ecoinvent v3, Allocation, cut-off by classification, Swiss Centre of Life Cycle Inventories.
Iversen et al., (2018) eEPD v3.0 - Background information for EPD generator system. LCA.no report number 04.18
Vold et al., (2019) EPD generator for Norsk Industri, Background information for industry application and LCA data, LCA.no report number 06.19.
NPCR Part A: Construction products and services. Ver. 1.0. April 2017, EPD-Norge.
NPCR 026 Part B for Furniture. Ver. 2.0 October 2018, EPD-Norge.
Program operator and publisher Phone: +47 23 08 80 00
The Norwegian EPD Foundation e-mail: post@epd-norge.no
Post Box 5250 Majorstuen, 0303 Oslo,Norway web: www.epd-norge.no
Owner of the declaration Phone: +370 657 52044
JSC Svenheim e-mail: info@svenheim.lt
Naujoji str.132 , LT-62175 Alytus web: www.svenheim.no
Author of the Life Cycle Assessment Phone: +47 916 50 916
LCA.no AS e-mail: post@lca.no
Dokka 1C , 1671 Kråkerøy web: www.lca.no
Developer of EPD generator Phone: +47 916 50 916
LCA.no AS e-mail: post@lca.no
Dokka 1C,1671 Kråkerøy web: www.lca.no
NEPD-2648-1355-EN Optima conference table 6000x1200 grey HPL 8 / 8
