ver1 2015
ENVIRONMENTAL PRODUCT DECLARATION
in accordance with ISO 14025, ISO 21930 and EN 15804
Owner of the declaration: Fora Form AS
Program operator: The Norwegian EPD Foundation
The Norwegian EPD Foundation
Publisher:
Declaration number: NEPD-2203-1001-EN
Registration number: NEPD-2203-1001-EN
ECO Platform reference number: -
Issue date: 26.05.2020
Valid to: 26.05.2025
Knekk stool
Fora Form AS
www.epd-norge.no
General information
Product: Owner of the declaration:
Knekk stool Fora Form AS
Contact person: Camilla Løseth
Phone: +47 700 46 000
e-mail: info@foraform.com
Program operator: Manufacturer:
The Norwegian EPD Foundation Fora Form AS
Pb. 5250 Majorstuen, 0303 Oslo
Phone: +47 97722020
e-mail: post@epd-norge.no
Declaration number: Place of production:
NEPD-2203-1001-EN Mosflatevegen
6154 Ørsta
N
ECO Platform reference number: Management system:
NS-EN ISO 14001: 2015 No. 800406. NS-EN ISO 9001: 2015 No.
901268. NS-EN ISO 45001: 2018 No 907167.
This declaration is based on Product Category Rules: Organisation no:
CEN Standard EN 15804:2012+A1:2013 serves as core PCR 986 581 421
PCR fot furniture NPCR 021 , Norwegian EPD Foundation
Statement of liability: Issue date: 26.05.2020
The owner of the declaration shall be liable for the underlying
information and evidence. EPD Norway shall not be liable with Valid to: 26.05.2025
respect to manufacturer information, life cycle assessment data and
evidences.
Declared unit: Year of study:
1 Pcs Knekk stool 2020
Declared unit with option: Comparability:
A1,A2,A3,A4 EPDs from programmes other than the Norwegian EPD Foundation
may not be comparable
Functional unit: Author of the Life Cycle Assessment:
The declaration is developed using eEPD v3.0 from LCA.no
Approval:
Company specific data are:
Collected/registered by: Kåre Sætre
Internal verification by: Camilla Løseth
Verification: Approved:
Independent verification of data, other environmental information and
the declaration according to ISO14025:2010, § 8.1.3 and § 8.1.4
Third party verifier:
Sign Sign
Seniorforsker Erik Svanes
(Independent verifier approved by EPD Norway)
Key environmental indicators Unit Cradle to gate A1 - A3
Global warming kg CO2 eqv 3,34
Total energy use MJ 134,25
Amount of recycled materials % 16,60
Product
Market: Technical data:
Dimensions: W: 46 cm H: 66 cm D: 53 cm SH: 66 cm
Worldwide
Weight : 5 kg ( packaging exluded )
Product description:
Reference service life, product
Interaction and function meet Nordic minimalism. The horizontal part of
the seat provides for reflection and relaxation. The askew part of the seat
gives direction for active interaction and support new and innovative
Reference service life, building
processes.
“Knekk” is a student work by Jon Fauske designed to capture Fora Form
values in a young and surprising fashion.
The modern designed solid wood stool is stackable with brass details.
Natural oak. Stackable. Brass cover on footrest.
Product specification
Recycled share in Recycled share in
Materials kg %
material (kg) material (%)
Metal - Brass 0,20 4,27 0,00 0,00
Plastic - Polyoxymethylene (POM) 0,01 0,13 0,00 50,00
Wood - Solid oak 4,40 93,90 0,00 0,00
Paint, water-based 0,40 1,71 0,00 0,00
Recycled share in Recycled share in
Packaging kg
material (kg) material (%)
Packaging - Cardboard 1,50 1,14 76,30
LCA: Calculation rules
Declared unit: Allocation:
The allocation is made in accordance with the provisions of EN 15804.
1 Pcs Knekk stool
Effects of primary production of recycled materials is allocated to the
Cut-off criteria: main product in which the material was used. The recycling process and
All major raw materials and all the essential energy is included. The transportation of the material is allocated to this analysis.
production processes for raw materials and energy flows with very small
amounts (less than 1%) are not included. These cut-off criteria do not
apply for hazardous materials and substances.
Data quality:
Specific data for the product composition are provided by the manufacturer. They represent the production of the declared product and were collected
for EPD development in the year of study. Background data is based on registered EPDs according to EN 15804, Ostfold Research databases,
ecoinvent and other LCA databases. The data quality of the raw materials in A1 is presented in the table below.
Materials Source Data quality Year
Plastic - Polyoxymethylene (POM) ecoinvent 3.4 Database 2015
Metal - Brass ecoinvent 3.4 Database 2017
Metal - Steel ecoinvent 3.4 Database 2017
Packaging - Cardboard ecoinvent 3.4 Database 2017
Paint, water-based ecoinvent 3.4 Database 2017
Plastics ecoinvent 3.4 Database 2017
Wood - Solid oak ecoinvent 3.4 Database 2017
System boundary:
Additional technical information:
The following information describe the scenarios in the different modules of the EPD.
The following information describe the scenarios in the different modules of the EPD.
Transport from production place to user (A4)
Capacity
Fuel/Energy
Type utilisation (incl. Type of vehicle Distance km Unit Value (l/t)
consumption
return) %
Truck, over 32
Truck 55,0 % 500 0,022823 l/tkm 11,41
tonnes, EURO 5
Railway l/tkm
Boat l/tkm
Other Transportation l/tkm
LCA: Results
System boundaries (X=included, MND=module not declared, MNR=module not relevant)
Construction Beyond the
Product stage installation User stage End of life stage . system
stage bondaries
A1 A2 A3 A4 A5 B1 B2 B3 B4 B5 B6 B7 C1 C2 C3 C4 . D
X X X X MND MND MND MND MND MND MNR MND MND MND MND MND . MND
Environmental impact
Parameter Unit A1 A2 A3 A4
GWP kg CO 2 -eq 3,34E+00 5,94E-01 7,76E-03 2,83E-01
ODP kg CFC11 -eq 2,86E-07 1,16E-07 7,34E-10 5,53E-08
POCP kg C 2H 4-eq 3,02E-03 9,61E-05 1,74E-06 4,58E-05
AP kg SO 2 -eq 6,61E-02 1,93E-03 3,62E-05 9,22E-04
EP kg PO3- -eq 1,76E-02 3,24E-04 8,73E-06 1,55E-04
4
ADPM kg Sb -eq 6,74E-04 1,34E-06 1,27E-07 6,40E-07
ADPE MJ 3,84E+01 9,33E+00 7,87E-02 4,45E+00
GWP Global warming potential; ODP Depletion potential of the stratospheric ozone layer; POCP Formation potential of tropospheric photochemical
oxidants; AP Acidification potential of land and water; EP Eutrophication potential; ADPM Abiotic depletion potential for non fossil resources; ADPE
Abiotic depletion potential for fossil resources
Reading example: 9,0 E-03 = 9,0*10-3 = 0,009
*INA Indicator Not Assessed
waR slairetam tropsnarT
gnirutcafunaM
tropsnarT ylbmessA esU ecnanetniaM riapeR tnemecalpeR
tnemhsibrufeR
lanoitarepO ygrene esu lanoitarepO esu retaw -eD noitcurtsnoc noitilomed tropsnarT etsaW gnissecorp lasopsiD
-yrevoceR-esueR
-gnilcyceR laitnetop
NEPD-2203-1001-EN Knekk stool 1 / 8
Resource use
Parameter Unit A1 A2 A3 A4
RPEE MJ 9,09E+01 1,69E-01 1,02E+00 8,04E-02
RPEM MJ 5,83E+01 0,00E+00 0,00E+00 0,00E+00
TPE MJ 1,49E+02 1,69E-01 1,02E+00 8,04E-02
NRPE MJ 4,33E+01 9,62E+00 1,35E-01 4,59E+00
NRPM MJ 1,11E-01 0,00E+00 0,00E+00 0,00E+00
TRPE MJ 4,34E+01 9,62E+00 1,35E-01 4,59E+00
SM kg 1,15E+00 0,00E+00 0,00E+00 0,00E+00
RSF MJ 0,00E+00 0,00E+00 1,77E-04 0,00E+00
NRSF MJ 0,00E+00 0,00E+00 0,00E+00 0,00E+00
W m3 6,72E-02 2,27E-03 5,65E-05 1,08E-03
RPEE Renewable primary energy resources used as energy carrier; RPEM Renewable primary energy resources used as raw materials; TPE Total use
of renewable primary energy resources; NRPE Non renewable primary energy resources used as energy carrier; NRPM Non renewable primary energy
resources used as materials; TRPE Total use of non renewable primary energy resources; SM Use of secondary materials; RSF Use of renewable
secondary fuels; NRSF Use of non renewable secondary fuels; W Use of net fresh water
Reading example: 9,0 E-03 = 9,0*10-3 = 0,009
*INA Indicator Not Assessed
End of life - Waste
Parameter Unit A1 A2 A3 A4
HW kg 2,47E-04 5,11E-06 1,74E-07 2,44E-06
NHW kg 5,98E+00 8,73E-01 1,03E-02 4,16E-01
RW kg INA* INA* INA* INA*
HW Hazardous waste disposed; NHW Non hazardous waste disposed; RW Radioactive waste disposed
Reading example: 9,0 E-03 = 9,0*10-3 = 0,009
*INA Indicator Not Assessed
End of life - Output flow
Parameter Unit A1 A2 A3 A4
CR kg 0,00E+00 0,00E+00 0,00E+00 0,00E+00
MR kg 0,00E+00 0,00E+00 0,00E+00 0,00E+00
MER kg 0,00E+00 0,00E+00 0,00E+00 0,00E+00
EEE MJ INA* INA* INA* INA*
ETE MJ INA* INA* INA* INA*
CR Components for reuse; MR Materials for recycling; MER Materials for energy recovery; EEE Exported electric energy; ETE Exported thermal
energy
Reading example: 9,0 E-03 = 9,0*10-3 = 0,009
*INA Indicator Not Assessed
Additional Norwegian requirements
Greenhouse gas emissions from the use of electricity in the manufacturing phase
National production mix from import, low voltage (production of transmission lines, in addition to direct emissions and losses in grid) of applied
electricity for the manufacturing process (A3).
Electricity mix Data source Amount Unit
El-mix, Norway (kWh) ecoinvent 3.4 31,04 g CO2-ekv/kWh
Dangerous substances
The product contains no substances given by the REACH Candidate list or the Norwegian priority list.
Indoor environment
Our furniture doesn't contain any substanses that effect indoor climate.
Additional environmental information
Bibliography
ISO 14025:2010 Environmental labels and declarations - Type III environmental declarations - Principles and procedures.
ISO 14044:2006 Environmental management - Life cycle assessment - Requirements and guidelines.
EN 15804:2012+A1:2013 Environmental product declaration - Core rules for the product category of construction products.
ISO 21930:2017 Sustainability in buildings and civil engineering works - Core rules for environmental product declarations of construction products.
ecoinvent v3, Allocation, cut-off by classification, Swiss Centre of Life Cycle Inventories.
Iversen et al., (2018) eEPD v3.0 - Background information for EPD generator system. LCA.no report number 04.18
Vold et al., (2019) EPD generator for Norsk Industri, Background information for industry application and LCA data, LCA.no report number 06.19.
NPCR Part A: Construction products and services. Ver. 1.0. April 2017, EPD-Norge.
NPCR 026 Part B for Furniture. Ver. 2.0 October 2018, EPD-Norge.
Program operator and publisher Phone: +47 97722020
The Norwegian EPD Foundation
Post Box 5250 Majorstuen, 0303 Oslo e-mail: post@epd-norge.no
0303 Oslo Norway web: www.epd-norge.no
Owner of the declaration Phone: +47 700 46 000
Fora Form AS Fax:
Mosfaltevegen e-mail: info@foraform.com
6154 Ørsta web: www.foraform.no
Author of the Life Cycle Assessment Phone: +47 916 50 916
LCA.no AS Fax:
Dokka 1C e-mail: post@lca.no
1671 Kråkerøy web: www.lca.no
Developer of EPD generator Phone: +47 916 50 916
LCA.no AS
Dokka 1C e-mail: post@lca.no
1671 Kråkerøy web: www.lca.no
ver1 2015
ENVIRONMENTAL PRODUCT DECLARATION
in accordance with ISO 14025, ISO 21930 and EN 15804
Owner of the declaration: Fora Form AS
Program operator: The Norwegian EPD Foundation
The Norwegian EPD Foundation
Publisher:
Declaration number: NEPD-2203-1001-EN
Registration number: NEPD-2203-1001-EN
ECO Platform reference number: -
Issue date: 26.05.2020
Valid to: 26.05.2025
Knekk stool
Fora Form AS
www.epd-norge.no
General information
Product: Owner of the declaration:
Knekk stool Fora Form AS
Contact person: Camilla Løseth
Phone: +47 700 46 000
e-mail: info@foraform.com
Program operator: Manufacturer:
The Norwegian EPD Foundation Fora Form AS
Pb. 5250 Majorstuen, 0303 Oslo
Phone: +47 97722020
e-mail: post@epd-norge.no
Declaration number: Place of production:
NEPD-2203-1001-EN Mosflatevegen
6154 Ørsta
N
ECO Platform reference number: Management system:
NS-EN ISO 14001: 2015 No. 800406. NS-EN ISO 9001: 2015 No.
901268. NS-EN ISO 45001: 2018 No 907167.
This declaration is based on Product Category Rules: Organisation no:
CEN Standard EN 15804:2012+A1:2013 serves as core PCR 986 581 421
PCR fot furniture NPCR 021 , Norwegian EPD Foundation
Statement of liability: Issue date: 26.05.2020
The owner of the declaration shall be liable for the underlying
information and evidence. EPD Norway shall not be liable with Valid to: 26.05.2025
respect to manufacturer information, life cycle assessment data and
evidences.
Declared unit: Year of study:
1 Pcs Knekk stool 2020
Declared unit with option: Comparability:
A1,A2,A3,A4 EPDs from programmes other than the Norwegian EPD Foundation
may not be comparable
Functional unit: Author of the Life Cycle Assessment:
The declaration is developed using eEPD v3.0 from LCA.no
Approval:
Company specific data are:
Collected/registered by: Kåre Sætre
Internal verification by: Camilla Løseth
Verification: Approved:
Independent verification of data, other environmental information and
the declaration according to ISO14025:2010, § 8.1.3 and § 8.1.4
Third party verifier:
Sign Sign
Seniorforsker Erik Svanes
(Independent verifier approved by EPD Norway)
Key environmental indicators Unit Cradle to gate A1 - A3
Global warming kg CO2 eqv 3,34
Total energy use MJ 134,25
Amount of recycled materials % 16,60
Product
Market: Technical data:
Dimensions: W: 46 cm H: 66 cm D: 53 cm SH: 66 cm
Worldwide
Weight : 5 kg ( packaging exluded )
Product description:
Reference service life, product
Interaction and function meet Nordic minimalism. The horizontal part of
the seat provides for reflection and relaxation. The askew part of the seat
gives direction for active interaction and support new and innovative
Reference service life, building
processes.
“Knekk” is a student work by Jon Fauske designed to capture Fora Form
values in a young and surprising fashion.
The modern designed solid wood stool is stackable with brass details.
Natural oak. Stackable. Brass cover on footrest.
Product specification
Recycled share in Recycled share in
Materials kg %
material (kg) material (%)
Metal - Brass 0,20 4,27 0,00 0,00
Plastic - Polyoxymethylene (POM) 0,01 0,13 0,00 50,00
Wood - Solid oak 4,40 93,90 0,00 0,00
Paint, water-based 0,40 1,71 0,00 0,00
Recycled share in Recycled share in
Packaging kg
material (kg) material (%)
Packaging - Cardboard 1,50 1,14 76,30
LCA: Calculation rules
Declared unit: Allocation:
The allocation is made in accordance with the provisions of EN 15804.
1 Pcs Knekk stool
Effects of primary production of recycled materials is allocated to the
Cut-off criteria: main product in which the material was used. The recycling process and
All major raw materials and all the essential energy is included. The transportation of the material is allocated to this analysis.
production processes for raw materials and energy flows with very small
amounts (less than 1%) are not included. These cut-off criteria do not
apply for hazardous materials and substances.
Data quality:
Specific data for the product composition are provided by the manufacturer. They represent the production of the declared product and were collected
for EPD development in the year of study. Background data is based on registered EPDs according to EN 15804, Ostfold Research databases,
ecoinvent and other LCA databases. The data quality of the raw materials in A1 is presented in the table below.
Materials Source Data quality Year
Plastic - Polyoxymethylene (POM) ecoinvent 3.4 Database 2015
Metal - Brass ecoinvent 3.4 Database 2017
Metal - Steel ecoinvent 3.4 Database 2017
Packaging - Cardboard ecoinvent 3.4 Database 2017
Paint, water-based ecoinvent 3.4 Database 2017
Plastics ecoinvent 3.4 Database 2017
Wood - Solid oak ecoinvent 3.4 Database 2017
System boundary:
Additional technical information:
The following information describe the scenarios in the different modules of the EPD.
The following information describe the scenarios in the different modules of the EPD.
Transport from production place to user (A4)
Capacity
Fuel/Energy
Type utilisation (incl. Type of vehicle Distance km Unit Value (l/t)
consumption
return) %
Truck, over 32
Truck 55,0 % 500 0,022823 l/tkm 11,41
tonnes, EURO 5
Railway l/tkm
Boat l/tkm
Other Transportation l/tkm
LCA: Results
System boundaries (X=included, MND=module not declared, MNR=module not relevant)
Construction Beyond the
Product stage installation User stage End of life stage . system
stage bondaries
A1 A2 A3 A4 A5 B1 B2 B3 B4 B5 B6 B7 C1 C2 C3 C4 . D
X X X X MND MND MND MND MND MND MNR MND MND MND MND MND . MND
Environmental impact
Parameter Unit A1 A2 A3 A4
GWP kg CO 2 -eq 3,34E+00 5,94E-01 7,76E-03 2,83E-01
ODP kg CFC11 -eq 2,86E-07 1,16E-07 7,34E-10 5,53E-08
POCP kg C 2H 4-eq 3,02E-03 9,61E-05 1,74E-06 4,58E-05
AP kg SO 2 -eq 6,61E-02 1,93E-03 3,62E-05 9,22E-04
EP kg PO3- -eq 1,76E-02 3,24E-04 8,73E-06 1,55E-04
4
ADPM kg Sb -eq 6,74E-04 1,34E-06 1,27E-07 6,40E-07
ADPE MJ 3,84E+01 9,33E+00 7,87E-02 4,45E+00
GWP Global warming potential; ODP Depletion potential of the stratospheric ozone layer; POCP Formation potential of tropospheric photochemical
oxidants; AP Acidification potential of land and water; EP Eutrophication potential; ADPM Abiotic depletion potential for non fossil resources; ADPE
Abiotic depletion potential for fossil resources
Reading example: 9,0 E-03 = 9,0*10-3 = 0,009
*INA Indicator Not Assessed
waR slairetam tropsnarT
gnirutcafunaM
tropsnarT ylbmessA esU ecnanetniaM riapeR tnemecalpeR
tnemhsibrufeR
lanoitarepO ygrene esu lanoitarepO esu retaw -eD noitcurtsnoc noitilomed tropsnarT etsaW gnissecorp lasopsiD
-yrevoceR-esueR
-gnilcyceR laitnetop
NEPD-2203-1001-EN Knekk stool 2 / 8
Resource use
Parameter Unit A1 A2 A3 A4
RPEE MJ 9,09E+01 1,69E-01 1,02E+00 8,04E-02
RPEM MJ 5,83E+01 0,00E+00 0,00E+00 0,00E+00
TPE MJ 1,49E+02 1,69E-01 1,02E+00 8,04E-02
NRPE MJ 4,33E+01 9,62E+00 1,35E-01 4,59E+00
NRPM MJ 1,11E-01 0,00E+00 0,00E+00 0,00E+00
TRPE MJ 4,34E+01 9,62E+00 1,35E-01 4,59E+00
SM kg 1,15E+00 0,00E+00 0,00E+00 0,00E+00
RSF MJ 0,00E+00 0,00E+00 1,77E-04 0,00E+00
NRSF MJ 0,00E+00 0,00E+00 0,00E+00 0,00E+00
W m3 6,72E-02 2,27E-03 5,65E-05 1,08E-03
RPEE Renewable primary energy resources used as energy carrier; RPEM Renewable primary energy resources used as raw materials; TPE Total use
of renewable primary energy resources; NRPE Non renewable primary energy resources used as energy carrier; NRPM Non renewable primary energy
resources used as materials; TRPE Total use of non renewable primary energy resources; SM Use of secondary materials; RSF Use of renewable
secondary fuels; NRSF Use of non renewable secondary fuels; W Use of net fresh water
Reading example: 9,0 E-03 = 9,0*10-3 = 0,009
*INA Indicator Not Assessed
End of life - Waste
Parameter Unit A1 A2 A3 A4
HW kg 2,47E-04 5,11E-06 1,74E-07 2,44E-06
NHW kg 5,98E+00 8,73E-01 1,03E-02 4,16E-01
RW kg INA* INA* INA* INA*
HW Hazardous waste disposed; NHW Non hazardous waste disposed; RW Radioactive waste disposed
Reading example: 9,0 E-03 = 9,0*10-3 = 0,009
*INA Indicator Not Assessed
End of life - Output flow
Parameter Unit A1 A2 A3 A4
CR kg 0,00E+00 0,00E+00 0,00E+00 0,00E+00
MR kg 0,00E+00 0,00E+00 0,00E+00 0,00E+00
MER kg 0,00E+00 0,00E+00 0,00E+00 0,00E+00
EEE MJ INA* INA* INA* INA*
ETE MJ INA* INA* INA* INA*
CR Components for reuse; MR Materials for recycling; MER Materials for energy recovery; EEE Exported electric energy; ETE Exported thermal
energy
Reading example: 9,0 E-03 = 9,0*10-3 = 0,009
*INA Indicator Not Assessed
Additional Norwegian requirements
Greenhouse gas emissions from the use of electricity in the manufacturing phase
National production mix from import, low voltage (production of transmission lines, in addition to direct emissions and losses in grid) of applied
electricity for the manufacturing process (A3).
Electricity mix Data source Amount Unit
El-mix, Norway (kWh) ecoinvent 3.4 31,04 g CO2-ekv/kWh
Dangerous substances
The product contains no substances given by the REACH Candidate list or the Norwegian priority list.
Indoor environment
Our furniture doesn't contain any substanses that effect indoor climate.
Additional environmental information
Bibliography
ISO 14025:2010 Environmental labels and declarations - Type III environmental declarations - Principles and procedures.
ISO 14044:2006 Environmental management - Life cycle assessment - Requirements and guidelines.
EN 15804:2012+A1:2013 Environmental product declaration - Core rules for the product category of construction products.
ISO 21930:2017 Sustainability in buildings and civil engineering works - Core rules for environmental product declarations of construction products.
ecoinvent v3, Allocation, cut-off by classification, Swiss Centre of Life Cycle Inventories.
Iversen et al., (2018) eEPD v3.0 - Background information for EPD generator system. LCA.no report number 04.18
Vold et al., (2019) EPD generator for Norsk Industri, Background information for industry application and LCA data, LCA.no report number 06.19.
NPCR Part A: Construction products and services. Ver. 1.0. April 2017, EPD-Norge.
NPCR 026 Part B for Furniture. Ver. 2.0 October 2018, EPD-Norge.
Program operator and publisher Phone: +47 97722020
The Norwegian EPD Foundation
Post Box 5250 Majorstuen, 0303 Oslo e-mail: post@epd-norge.no
0303 Oslo Norway web: www.epd-norge.no
Owner of the declaration Phone: +47 700 46 000
Fora Form AS Fax:
Mosfaltevegen e-mail: info@foraform.com
6154 Ørsta web: www.foraform.no
Author of the Life Cycle Assessment Phone: +47 916 50 916
LCA.no AS Fax:
Dokka 1C e-mail: post@lca.no
1671 Kråkerøy web: www.lca.no
Developer of EPD generator Phone: +47 916 50 916
LCA.no AS
Dokka 1C e-mail: post@lca.no
1671 Kråkerøy web: www.lca.no
ver1 2015
ENVIRONMENTAL PRODUCT DECLARATION
in accordance with ISO 14025, ISO 21930 and EN 15804
Owner of the declaration: Fora Form AS
Program operator: The Norwegian EPD Foundation
The Norwegian EPD Foundation
Publisher:
Declaration number: NEPD-2203-1001-EN
Registration number: NEPD-2203-1001-EN
ECO Platform reference number: -
Issue date: 26.05.2020
Valid to: 26.05.2025
Knekk stool
Fora Form AS
www.epd-norge.no
General information
Product: Owner of the declaration:
Knekk stool Fora Form AS
Contact person: Camilla Løseth
Phone: +47 700 46 000
e-mail: info@foraform.com
Program operator: Manufacturer:
The Norwegian EPD Foundation Fora Form AS
Pb. 5250 Majorstuen, 0303 Oslo
Phone: +47 97722020
e-mail: post@epd-norge.no
Declaration number: Place of production:
NEPD-2203-1001-EN Mosflatevegen
6154 Ørsta
N
ECO Platform reference number: Management system:
NS-EN ISO 14001: 2015 No. 800406. NS-EN ISO 9001: 2015 No.
901268. NS-EN ISO 45001: 2018 No 907167.
This declaration is based on Product Category Rules: Organisation no:
CEN Standard EN 15804:2012+A1:2013 serves as core PCR 986 581 421
PCR fot furniture NPCR 021 , Norwegian EPD Foundation
Statement of liability: Issue date: 26.05.2020
The owner of the declaration shall be liable for the underlying
information and evidence. EPD Norway shall not be liable with Valid to: 26.05.2025
respect to manufacturer information, life cycle assessment data and
evidences.
Declared unit: Year of study:
1 Pcs Knekk stool 2020
Declared unit with option: Comparability:
A1,A2,A3,A4 EPDs from programmes other than the Norwegian EPD Foundation
may not be comparable
Functional unit: Author of the Life Cycle Assessment:
The declaration is developed using eEPD v3.0 from LCA.no
Approval:
Company specific data are:
Collected/registered by: Kåre Sætre
Internal verification by: Camilla Løseth
Verification: Approved:
Independent verification of data, other environmental information and
the declaration according to ISO14025:2010, § 8.1.3 and § 8.1.4
Third party verifier:
Sign Sign
Seniorforsker Erik Svanes
(Independent verifier approved by EPD Norway)
Key environmental indicators Unit Cradle to gate A1 - A3
Global warming kg CO2 eqv 3,34
Total energy use MJ 134,25
Amount of recycled materials % 16,60
Product
Market: Technical data:
Dimensions: W: 46 cm H: 66 cm D: 53 cm SH: 66 cm
Worldwide
Weight : 5 kg ( packaging exluded )
Product description:
Reference service life, product
Interaction and function meet Nordic minimalism. The horizontal part of
the seat provides for reflection and relaxation. The askew part of the seat
gives direction for active interaction and support new and innovative
Reference service life, building
processes.
“Knekk” is a student work by Jon Fauske designed to capture Fora Form
values in a young and surprising fashion.
The modern designed solid wood stool is stackable with brass details.
Natural oak. Stackable. Brass cover on footrest.
Product specification
Recycled share in Recycled share in
Materials kg %
material (kg) material (%)
Metal - Brass 0,20 4,27 0,00 0,00
Plastic - Polyoxymethylene (POM) 0,01 0,13 0,00 50,00
Wood - Solid oak 4,40 93,90 0,00 0,00
Paint, water-based 0,40 1,71 0,00 0,00
Recycled share in Recycled share in
Packaging kg
material (kg) material (%)
Packaging - Cardboard 1,50 1,14 76,30
LCA: Calculation rules
Declared unit: Allocation:
The allocation is made in accordance with the provisions of EN 15804.
1 Pcs Knekk stool
Effects of primary production of recycled materials is allocated to the
Cut-off criteria: main product in which the material was used. The recycling process and
All major raw materials and all the essential energy is included. The transportation of the material is allocated to this analysis.
production processes for raw materials and energy flows with very small
amounts (less than 1%) are not included. These cut-off criteria do not
apply for hazardous materials and substances.
Data quality:
Specific data for the product composition are provided by the manufacturer. They represent the production of the declared product and were collected
for EPD development in the year of study. Background data is based on registered EPDs according to EN 15804, Ostfold Research databases,
ecoinvent and other LCA databases. The data quality of the raw materials in A1 is presented in the table below.
Materials Source Data quality Year
Plastic - Polyoxymethylene (POM) ecoinvent 3.4 Database 2015
Metal - Brass ecoinvent 3.4 Database 2017
Metal - Steel ecoinvent 3.4 Database 2017
Packaging - Cardboard ecoinvent 3.4 Database 2017
Paint, water-based ecoinvent 3.4 Database 2017
Plastics ecoinvent 3.4 Database 2017
Wood - Solid oak ecoinvent 3.4 Database 2017
System boundary:
Additional technical information:
The following information describe the scenarios in the different modules of the EPD.
The following information describe the scenarios in the different modules of the EPD.
Transport from production place to user (A4)
Capacity
Fuel/Energy
Type utilisation (incl. Type of vehicle Distance km Unit Value (l/t)
consumption
return) %
Truck, over 32
Truck 55,0 % 500 0,022823 l/tkm 11,41
tonnes, EURO 5
Railway l/tkm
Boat l/tkm
Other Transportation l/tkm
LCA: Results
System boundaries (X=included, MND=module not declared, MNR=module not relevant)
Construction Beyond the
Product stage installation User stage End of life stage . system
stage bondaries
A1 A2 A3 A4 A5 B1 B2 B3 B4 B5 B6 B7 C1 C2 C3 C4 . D
X X X X MND MND MND MND MND MND MNR MND MND MND MND MND . MND
Environmental impact
Parameter Unit A1 A2 A3 A4
GWP kg CO 2 -eq 3,34E+00 5,94E-01 7,76E-03 2,83E-01
ODP kg CFC11 -eq 2,86E-07 1,16E-07 7,34E-10 5,53E-08
POCP kg C 2H 4-eq 3,02E-03 9,61E-05 1,74E-06 4,58E-05
AP kg SO 2 -eq 6,61E-02 1,93E-03 3,62E-05 9,22E-04
EP kg PO3- -eq 1,76E-02 3,24E-04 8,73E-06 1,55E-04
4
ADPM kg Sb -eq 6,74E-04 1,34E-06 1,27E-07 6,40E-07
ADPE MJ 3,84E+01 9,33E+00 7,87E-02 4,45E+00
GWP Global warming potential; ODP Depletion potential of the stratospheric ozone layer; POCP Formation potential of tropospheric photochemical
oxidants; AP Acidification potential of land and water; EP Eutrophication potential; ADPM Abiotic depletion potential for non fossil resources; ADPE
Abiotic depletion potential for fossil resources
Reading example: 9,0 E-03 = 9,0*10-3 = 0,009
*INA Indicator Not Assessed
waR slairetam tropsnarT
gnirutcafunaM
tropsnarT ylbmessA esU ecnanetniaM riapeR tnemecalpeR
tnemhsibrufeR
lanoitarepO ygrene esu lanoitarepO esu retaw -eD noitcurtsnoc noitilomed tropsnarT etsaW gnissecorp lasopsiD
-yrevoceR-esueR
-gnilcyceR laitnetop
NEPD-2203-1001-EN Knekk stool 3 / 8
Resource use
Parameter Unit A1 A2 A3 A4
RPEE MJ 9,09E+01 1,69E-01 1,02E+00 8,04E-02
RPEM MJ 5,83E+01 0,00E+00 0,00E+00 0,00E+00
TPE MJ 1,49E+02 1,69E-01 1,02E+00 8,04E-02
NRPE MJ 4,33E+01 9,62E+00 1,35E-01 4,59E+00
NRPM MJ 1,11E-01 0,00E+00 0,00E+00 0,00E+00
TRPE MJ 4,34E+01 9,62E+00 1,35E-01 4,59E+00
SM kg 1,15E+00 0,00E+00 0,00E+00 0,00E+00
RSF MJ 0,00E+00 0,00E+00 1,77E-04 0,00E+00
NRSF MJ 0,00E+00 0,00E+00 0,00E+00 0,00E+00
W m3 6,72E-02 2,27E-03 5,65E-05 1,08E-03
RPEE Renewable primary energy resources used as energy carrier; RPEM Renewable primary energy resources used as raw materials; TPE Total use
of renewable primary energy resources; NRPE Non renewable primary energy resources used as energy carrier; NRPM Non renewable primary energy
resources used as materials; TRPE Total use of non renewable primary energy resources; SM Use of secondary materials; RSF Use of renewable
secondary fuels; NRSF Use of non renewable secondary fuels; W Use of net fresh water
Reading example: 9,0 E-03 = 9,0*10-3 = 0,009
*INA Indicator Not Assessed
End of life - Waste
Parameter Unit A1 A2 A3 A4
HW kg 2,47E-04 5,11E-06 1,74E-07 2,44E-06
NHW kg 5,98E+00 8,73E-01 1,03E-02 4,16E-01
RW kg INA* INA* INA* INA*
HW Hazardous waste disposed; NHW Non hazardous waste disposed; RW Radioactive waste disposed
Reading example: 9,0 E-03 = 9,0*10-3 = 0,009
*INA Indicator Not Assessed
End of life - Output flow
Parameter Unit A1 A2 A3 A4
CR kg 0,00E+00 0,00E+00 0,00E+00 0,00E+00
MR kg 0,00E+00 0,00E+00 0,00E+00 0,00E+00
MER kg 0,00E+00 0,00E+00 0,00E+00 0,00E+00
EEE MJ INA* INA* INA* INA*
ETE MJ INA* INA* INA* INA*
CR Components for reuse; MR Materials for recycling; MER Materials for energy recovery; EEE Exported electric energy; ETE Exported thermal
energy
Reading example: 9,0 E-03 = 9,0*10-3 = 0,009
*INA Indicator Not Assessed
Additional Norwegian requirements
Greenhouse gas emissions from the use of electricity in the manufacturing phase
National production mix from import, low voltage (production of transmission lines, in addition to direct emissions and losses in grid) of applied
electricity for the manufacturing process (A3).
Electricity mix Data source Amount Unit
El-mix, Norway (kWh) ecoinvent 3.4 31,04 g CO2-ekv/kWh
Dangerous substances
The product contains no substances given by the REACH Candidate list or the Norwegian priority list.
Indoor environment
Our furniture doesn't contain any substanses that effect indoor climate.
Additional environmental information
Bibliography
ISO 14025:2010 Environmental labels and declarations - Type III environmental declarations - Principles and procedures.
ISO 14044:2006 Environmental management - Life cycle assessment - Requirements and guidelines.
EN 15804:2012+A1:2013 Environmental product declaration - Core rules for the product category of construction products.
ISO 21930:2017 Sustainability in buildings and civil engineering works - Core rules for environmental product declarations of construction products.
ecoinvent v3, Allocation, cut-off by classification, Swiss Centre of Life Cycle Inventories.
Iversen et al., (2018) eEPD v3.0 - Background information for EPD generator system. LCA.no report number 04.18
Vold et al., (2019) EPD generator for Norsk Industri, Background information for industry application and LCA data, LCA.no report number 06.19.
NPCR Part A: Construction products and services. Ver. 1.0. April 2017, EPD-Norge.
NPCR 026 Part B for Furniture. Ver. 2.0 October 2018, EPD-Norge.
Program operator and publisher Phone: +47 97722020
The Norwegian EPD Foundation
Post Box 5250 Majorstuen, 0303 Oslo e-mail: post@epd-norge.no
0303 Oslo Norway web: www.epd-norge.no
Owner of the declaration Phone: +47 700 46 000
Fora Form AS Fax:
Mosfaltevegen e-mail: info@foraform.com
6154 Ørsta web: www.foraform.no
Author of the Life Cycle Assessment Phone: +47 916 50 916
LCA.no AS Fax:
Dokka 1C e-mail: post@lca.no
1671 Kråkerøy web: www.lca.no
Developer of EPD generator Phone: +47 916 50 916
LCA.no AS
Dokka 1C e-mail: post@lca.no
1671 Kråkerøy web: www.lca.no
ver1 2015
ENVIRONMENTAL PRODUCT DECLARATION
in accordance with ISO 14025, ISO 21930 and EN 15804
Owner of the declaration: Fora Form AS
Program operator: The Norwegian EPD Foundation
The Norwegian EPD Foundation
Publisher:
Declaration number: NEPD-2203-1001-EN
Registration number: NEPD-2203-1001-EN
ECO Platform reference number: -
Issue date: 26.05.2020
Valid to: 26.05.2025
Knekk stool
Fora Form AS
www.epd-norge.no
General information
Product: Owner of the declaration:
Knekk stool Fora Form AS
Contact person: Camilla Løseth
Phone: +47 700 46 000
e-mail: info@foraform.com
Program operator: Manufacturer:
The Norwegian EPD Foundation Fora Form AS
Pb. 5250 Majorstuen, 0303 Oslo
Phone: +47 97722020
e-mail: post@epd-norge.no
Declaration number: Place of production:
NEPD-2203-1001-EN Mosflatevegen
6154 Ørsta
N
ECO Platform reference number: Management system:
NS-EN ISO 14001: 2015 No. 800406. NS-EN ISO 9001: 2015 No.
901268. NS-EN ISO 45001: 2018 No 907167.
This declaration is based on Product Category Rules: Organisation no:
CEN Standard EN 15804:2012+A1:2013 serves as core PCR 986 581 421
PCR fot furniture NPCR 021 , Norwegian EPD Foundation
Statement of liability: Issue date: 26.05.2020
The owner of the declaration shall be liable for the underlying
information and evidence. EPD Norway shall not be liable with Valid to: 26.05.2025
respect to manufacturer information, life cycle assessment data and
evidences.
Declared unit: Year of study:
1 Pcs Knekk stool 2020
Declared unit with option: Comparability:
A1,A2,A3,A4 EPDs from programmes other than the Norwegian EPD Foundation
may not be comparable
Functional unit: Author of the Life Cycle Assessment:
The declaration is developed using eEPD v3.0 from LCA.no
Approval:
Company specific data are:
Collected/registered by: Kåre Sætre
Internal verification by: Camilla Løseth
Verification: Approved:
Independent verification of data, other environmental information and
the declaration according to ISO14025:2010, § 8.1.3 and § 8.1.4
Third party verifier:
Sign Sign
Seniorforsker Erik Svanes
(Independent verifier approved by EPD Norway)
Key environmental indicators Unit Cradle to gate A1 - A3
Global warming kg CO2 eqv 3,34
Total energy use MJ 134,25
Amount of recycled materials % 16,60
Product
Market: Technical data:
Dimensions: W: 46 cm H: 66 cm D: 53 cm SH: 66 cm
Worldwide
Weight : 5 kg ( packaging exluded )
Product description:
Reference service life, product
Interaction and function meet Nordic minimalism. The horizontal part of
the seat provides for reflection and relaxation. The askew part of the seat
gives direction for active interaction and support new and innovative
Reference service life, building
processes.
“Knekk” is a student work by Jon Fauske designed to capture Fora Form
values in a young and surprising fashion.
The modern designed solid wood stool is stackable with brass details.
Natural oak. Stackable. Brass cover on footrest.
Product specification
Recycled share in Recycled share in
Materials kg %
material (kg) material (%)
Metal - Brass 0,20 4,27 0,00 0,00
Plastic - Polyoxymethylene (POM) 0,01 0,13 0,00 50,00
Wood - Solid oak 4,40 93,90 0,00 0,00
Paint, water-based 0,40 1,71 0,00 0,00
Recycled share in Recycled share in
Packaging kg
material (kg) material (%)
Packaging - Cardboard 1,50 1,14 76,30
LCA: Calculation rules
Declared unit: Allocation:
The allocation is made in accordance with the provisions of EN 15804.
1 Pcs Knekk stool
Effects of primary production of recycled materials is allocated to the
Cut-off criteria: main product in which the material was used. The recycling process and
All major raw materials and all the essential energy is included. The transportation of the material is allocated to this analysis.
production processes for raw materials and energy flows with very small
amounts (less than 1%) are not included. These cut-off criteria do not
apply for hazardous materials and substances.
Data quality:
Specific data for the product composition are provided by the manufacturer. They represent the production of the declared product and were collected
for EPD development in the year of study. Background data is based on registered EPDs according to EN 15804, Ostfold Research databases,
ecoinvent and other LCA databases. The data quality of the raw materials in A1 is presented in the table below.
Materials Source Data quality Year
Plastic - Polyoxymethylene (POM) ecoinvent 3.4 Database 2015
Metal - Brass ecoinvent 3.4 Database 2017
Metal - Steel ecoinvent 3.4 Database 2017
Packaging - Cardboard ecoinvent 3.4 Database 2017
Paint, water-based ecoinvent 3.4 Database 2017
Plastics ecoinvent 3.4 Database 2017
Wood - Solid oak ecoinvent 3.4 Database 2017
System boundary:
Additional technical information:
The following information describe the scenarios in the different modules of the EPD.
The following information describe the scenarios in the different modules of the EPD.
Transport from production place to user (A4)
Capacity
Fuel/Energy
Type utilisation (incl. Type of vehicle Distance km Unit Value (l/t)
consumption
return) %
Truck, over 32
Truck 55,0 % 500 0,022823 l/tkm 11,41
tonnes, EURO 5
Railway l/tkm
Boat l/tkm
Other Transportation l/tkm
LCA: Results
System boundaries (X=included, MND=module not declared, MNR=module not relevant)
Construction Beyond the
Product stage installation User stage End of life stage . system
stage bondaries
A1 A2 A3 A4 A5 B1 B2 B3 B4 B5 B6 B7 C1 C2 C3 C4 . D
X X X X MND MND MND MND MND MND MNR MND MND MND MND MND . MND
Environmental impact
Parameter Unit A1 A2 A3 A4
GWP kg CO 2 -eq 3,34E+00 5,94E-01 7,76E-03 2,83E-01
ODP kg CFC11 -eq 2,86E-07 1,16E-07 7,34E-10 5,53E-08
POCP kg C 2H 4-eq 3,02E-03 9,61E-05 1,74E-06 4,58E-05
AP kg SO 2 -eq 6,61E-02 1,93E-03 3,62E-05 9,22E-04
EP kg PO3- -eq 1,76E-02 3,24E-04 8,73E-06 1,55E-04
4
ADPM kg Sb -eq 6,74E-04 1,34E-06 1,27E-07 6,40E-07
ADPE MJ 3,84E+01 9,33E+00 7,87E-02 4,45E+00
GWP Global warming potential; ODP Depletion potential of the stratospheric ozone layer; POCP Formation potential of tropospheric photochemical
oxidants; AP Acidification potential of land and water; EP Eutrophication potential; ADPM Abiotic depletion potential for non fossil resources; ADPE
Abiotic depletion potential for fossil resources
Reading example: 9,0 E-03 = 9,0*10-3 = 0,009
*INA Indicator Not Assessed
waR slairetam tropsnarT
gnirutcafunaM
tropsnarT ylbmessA esU ecnanetniaM riapeR tnemecalpeR
tnemhsibrufeR
lanoitarepO ygrene esu lanoitarepO esu retaw -eD noitcurtsnoc noitilomed tropsnarT etsaW gnissecorp lasopsiD
-yrevoceR-esueR
-gnilcyceR laitnetop
NEPD-2203-1001-EN Knekk stool 4 / 8
Resource use
Parameter Unit A1 A2 A3 A4
RPEE MJ 9,09E+01 1,69E-01 1,02E+00 8,04E-02
RPEM MJ 5,83E+01 0,00E+00 0,00E+00 0,00E+00
TPE MJ 1,49E+02 1,69E-01 1,02E+00 8,04E-02
NRPE MJ 4,33E+01 9,62E+00 1,35E-01 4,59E+00
NRPM MJ 1,11E-01 0,00E+00 0,00E+00 0,00E+00
TRPE MJ 4,34E+01 9,62E+00 1,35E-01 4,59E+00
SM kg 1,15E+00 0,00E+00 0,00E+00 0,00E+00
RSF MJ 0,00E+00 0,00E+00 1,77E-04 0,00E+00
NRSF MJ 0,00E+00 0,00E+00 0,00E+00 0,00E+00
W m3 6,72E-02 2,27E-03 5,65E-05 1,08E-03
RPEE Renewable primary energy resources used as energy carrier; RPEM Renewable primary energy resources used as raw materials; TPE Total use
of renewable primary energy resources; NRPE Non renewable primary energy resources used as energy carrier; NRPM Non renewable primary energy
resources used as materials; TRPE Total use of non renewable primary energy resources; SM Use of secondary materials; RSF Use of renewable
secondary fuels; NRSF Use of non renewable secondary fuels; W Use of net fresh water
Reading example: 9,0 E-03 = 9,0*10-3 = 0,009
*INA Indicator Not Assessed
End of life - Waste
Parameter Unit A1 A2 A3 A4
HW kg 2,47E-04 5,11E-06 1,74E-07 2,44E-06
NHW kg 5,98E+00 8,73E-01 1,03E-02 4,16E-01
RW kg INA* INA* INA* INA*
HW Hazardous waste disposed; NHW Non hazardous waste disposed; RW Radioactive waste disposed
Reading example: 9,0 E-03 = 9,0*10-3 = 0,009
*INA Indicator Not Assessed
End of life - Output flow
Parameter Unit A1 A2 A3 A4
CR kg 0,00E+00 0,00E+00 0,00E+00 0,00E+00
MR kg 0,00E+00 0,00E+00 0,00E+00 0,00E+00
MER kg 0,00E+00 0,00E+00 0,00E+00 0,00E+00
EEE MJ INA* INA* INA* INA*
ETE MJ INA* INA* INA* INA*
CR Components for reuse; MR Materials for recycling; MER Materials for energy recovery; EEE Exported electric energy; ETE Exported thermal
energy
Reading example: 9,0 E-03 = 9,0*10-3 = 0,009
*INA Indicator Not Assessed
Additional Norwegian requirements
Greenhouse gas emissions from the use of electricity in the manufacturing phase
National production mix from import, low voltage (production of transmission lines, in addition to direct emissions and losses in grid) of applied
electricity for the manufacturing process (A3).
Electricity mix Data source Amount Unit
El-mix, Norway (kWh) ecoinvent 3.4 31,04 g CO2-ekv/kWh
Dangerous substances
The product contains no substances given by the REACH Candidate list or the Norwegian priority list.
Indoor environment
Our furniture doesn't contain any substanses that effect indoor climate.
Additional environmental information
Bibliography
ISO 14025:2010 Environmental labels and declarations - Type III environmental declarations - Principles and procedures.
ISO 14044:2006 Environmental management - Life cycle assessment - Requirements and guidelines.
EN 15804:2012+A1:2013 Environmental product declaration - Core rules for the product category of construction products.
ISO 21930:2017 Sustainability in buildings and civil engineering works - Core rules for environmental product declarations of construction products.
ecoinvent v3, Allocation, cut-off by classification, Swiss Centre of Life Cycle Inventories.
Iversen et al., (2018) eEPD v3.0 - Background information for EPD generator system. LCA.no report number 04.18
Vold et al., (2019) EPD generator for Norsk Industri, Background information for industry application and LCA data, LCA.no report number 06.19.
NPCR Part A: Construction products and services. Ver. 1.0. April 2017, EPD-Norge.
NPCR 026 Part B for Furniture. Ver. 2.0 October 2018, EPD-Norge.
Program operator and publisher Phone: +47 97722020
The Norwegian EPD Foundation
Post Box 5250 Majorstuen, 0303 Oslo e-mail: post@epd-norge.no
0303 Oslo Norway web: www.epd-norge.no
Owner of the declaration Phone: +47 700 46 000
Fora Form AS Fax:
Mosfaltevegen e-mail: info@foraform.com
6154 Ørsta web: www.foraform.no
Author of the Life Cycle Assessment Phone: +47 916 50 916
LCA.no AS Fax:
Dokka 1C e-mail: post@lca.no
1671 Kråkerøy web: www.lca.no
Developer of EPD generator Phone: +47 916 50 916
LCA.no AS
Dokka 1C e-mail: post@lca.no
1671 Kråkerøy web: www.lca.no
ver1 2015
ENVIRONMENTAL PRODUCT DECLARATION
in accordance with ISO 14025, ISO 21930 and EN 15804
Owner of the declaration: Fora Form AS
Program operator: The Norwegian EPD Foundation
The Norwegian EPD Foundation
Publisher:
Declaration number: NEPD-2203-1001-EN
Registration number: NEPD-2203-1001-EN
ECO Platform reference number: -
Issue date: 26.05.2020
Valid to: 26.05.2025
Knekk stool
Fora Form AS
www.epd-norge.no
General information
Product: Owner of the declaration:
Knekk stool Fora Form AS
Contact person: Camilla Løseth
Phone: +47 700 46 000
e-mail: info@foraform.com
Program operator: Manufacturer:
The Norwegian EPD Foundation Fora Form AS
Pb. 5250 Majorstuen, 0303 Oslo
Phone: +47 97722020
e-mail: post@epd-norge.no
Declaration number: Place of production:
NEPD-2203-1001-EN Mosflatevegen
6154 Ørsta
N
ECO Platform reference number: Management system:
NS-EN ISO 14001: 2015 No. 800406. NS-EN ISO 9001: 2015 No.
901268. NS-EN ISO 45001: 2018 No 907167.
This declaration is based on Product Category Rules: Organisation no:
CEN Standard EN 15804:2012+A1:2013 serves as core PCR 986 581 421
PCR fot furniture NPCR 021 , Norwegian EPD Foundation
Statement of liability: Issue date: 26.05.2020
The owner of the declaration shall be liable for the underlying
information and evidence. EPD Norway shall not be liable with Valid to: 26.05.2025
respect to manufacturer information, life cycle assessment data and
evidences.
Declared unit: Year of study:
1 Pcs Knekk stool 2020
Declared unit with option: Comparability:
A1,A2,A3,A4 EPDs from programmes other than the Norwegian EPD Foundation
may not be comparable
Functional unit: Author of the Life Cycle Assessment:
The declaration is developed using eEPD v3.0 from LCA.no
Approval:
Company specific data are:
Collected/registered by: Kåre Sætre
Internal verification by: Camilla Løseth
Verification: Approved:
Independent verification of data, other environmental information and
the declaration according to ISO14025:2010, § 8.1.3 and § 8.1.4
Third party verifier:
Sign Sign
Seniorforsker Erik Svanes
(Independent verifier approved by EPD Norway)
Key environmental indicators Unit Cradle to gate A1 - A3
Global warming kg CO2 eqv 3,34
Total energy use MJ 134,25
Amount of recycled materials % 16,60
Product
Market: Technical data:
Dimensions: W: 46 cm H: 66 cm D: 53 cm SH: 66 cm
Worldwide
Weight : 5 kg ( packaging exluded )
Product description:
Reference service life, product
Interaction and function meet Nordic minimalism. The horizontal part of
the seat provides for reflection and relaxation. The askew part of the seat
gives direction for active interaction and support new and innovative
Reference service life, building
processes.
“Knekk” is a student work by Jon Fauske designed to capture Fora Form
values in a young and surprising fashion.
The modern designed solid wood stool is stackable with brass details.
Natural oak. Stackable. Brass cover on footrest.
Product specification
Recycled share in Recycled share in
Materials kg %
material (kg) material (%)
Metal - Brass 0,20 4,27 0,00 0,00
Plastic - Polyoxymethylene (POM) 0,01 0,13 0,00 50,00
Wood - Solid oak 4,40 93,90 0,00 0,00
Paint, water-based 0,40 1,71 0,00 0,00
Recycled share in Recycled share in
Packaging kg
material (kg) material (%)
Packaging - Cardboard 1,50 1,14 76,30
LCA: Calculation rules
Declared unit: Allocation:
The allocation is made in accordance with the provisions of EN 15804.
1 Pcs Knekk stool
Effects of primary production of recycled materials is allocated to the
Cut-off criteria: main product in which the material was used. The recycling process and
All major raw materials and all the essential energy is included. The transportation of the material is allocated to this analysis.
production processes for raw materials and energy flows with very small
amounts (less than 1%) are not included. These cut-off criteria do not
apply for hazardous materials and substances.
Data quality:
Specific data for the product composition are provided by the manufacturer. They represent the production of the declared product and were collected
for EPD development in the year of study. Background data is based on registered EPDs according to EN 15804, Ostfold Research databases,
ecoinvent and other LCA databases. The data quality of the raw materials in A1 is presented in the table below.
Materials Source Data quality Year
Plastic - Polyoxymethylene (POM) ecoinvent 3.4 Database 2015
Metal - Brass ecoinvent 3.4 Database 2017
Metal - Steel ecoinvent 3.4 Database 2017
Packaging - Cardboard ecoinvent 3.4 Database 2017
Paint, water-based ecoinvent 3.4 Database 2017
Plastics ecoinvent 3.4 Database 2017
Wood - Solid oak ecoinvent 3.4 Database 2017
System boundary:
Additional technical information:
The following information describe the scenarios in the different modules of the EPD.
The following information describe the scenarios in the different modules of the EPD.
Transport from production place to user (A4)
Capacity
Fuel/Energy
Type utilisation (incl. Type of vehicle Distance km Unit Value (l/t)
consumption
return) %
Truck, over 32
Truck 55,0 % 500 0,022823 l/tkm 11,41
tonnes, EURO 5
Railway l/tkm
Boat l/tkm
Other Transportation l/tkm
LCA: Results
System boundaries (X=included, MND=module not declared, MNR=module not relevant)
Construction Beyond the
Product stage installation User stage End of life stage . system
stage bondaries
A1 A2 A3 A4 A5 B1 B2 B3 B4 B5 B6 B7 C1 C2 C3 C4 . D
X X X X MND MND MND MND MND MND MNR MND MND MND MND MND . MND
Environmental impact
Parameter Unit A1 A2 A3 A4
GWP kg CO 2 -eq 3,34E+00 5,94E-01 7,76E-03 2,83E-01
ODP kg CFC11 -eq 2,86E-07 1,16E-07 7,34E-10 5,53E-08
POCP kg C 2H 4-eq 3,02E-03 9,61E-05 1,74E-06 4,58E-05
AP kg SO 2 -eq 6,61E-02 1,93E-03 3,62E-05 9,22E-04
EP kg PO3- -eq 1,76E-02 3,24E-04 8,73E-06 1,55E-04
4
ADPM kg Sb -eq 6,74E-04 1,34E-06 1,27E-07 6,40E-07
ADPE MJ 3,84E+01 9,33E+00 7,87E-02 4,45E+00
GWP Global warming potential; ODP Depletion potential of the stratospheric ozone layer; POCP Formation potential of tropospheric photochemical
oxidants; AP Acidification potential of land and water; EP Eutrophication potential; ADPM Abiotic depletion potential for non fossil resources; ADPE
Abiotic depletion potential for fossil resources
Reading example: 9,0 E-03 = 9,0*10-3 = 0,009
*INA Indicator Not Assessed
waR slairetam tropsnarT
gnirutcafunaM
tropsnarT ylbmessA esU ecnanetniaM riapeR tnemecalpeR
tnemhsibrufeR
lanoitarepO ygrene esu lanoitarepO esu retaw -eD noitcurtsnoc noitilomed tropsnarT etsaW gnissecorp lasopsiD
-yrevoceR-esueR
-gnilcyceR laitnetop
NEPD-2203-1001-EN Knekk stool 5 / 8
Resource use
Parameter Unit A1 A2 A3 A4
RPEE MJ 9,09E+01 1,69E-01 1,02E+00 8,04E-02
RPEM MJ 5,83E+01 0,00E+00 0,00E+00 0,00E+00
TPE MJ 1,49E+02 1,69E-01 1,02E+00 8,04E-02
NRPE MJ 4,33E+01 9,62E+00 1,35E-01 4,59E+00
NRPM MJ 1,11E-01 0,00E+00 0,00E+00 0,00E+00
TRPE MJ 4,34E+01 9,62E+00 1,35E-01 4,59E+00
SM kg 1,15E+00 0,00E+00 0,00E+00 0,00E+00
RSF MJ 0,00E+00 0,00E+00 1,77E-04 0,00E+00
NRSF MJ 0,00E+00 0,00E+00 0,00E+00 0,00E+00
W m3 6,72E-02 2,27E-03 5,65E-05 1,08E-03
RPEE Renewable primary energy resources used as energy carrier; RPEM Renewable primary energy resources used as raw materials; TPE Total use
of renewable primary energy resources; NRPE Non renewable primary energy resources used as energy carrier; NRPM Non renewable primary energy
resources used as materials; TRPE Total use of non renewable primary energy resources; SM Use of secondary materials; RSF Use of renewable
secondary fuels; NRSF Use of non renewable secondary fuels; W Use of net fresh water
Reading example: 9,0 E-03 = 9,0*10-3 = 0,009
*INA Indicator Not Assessed
End of life - Waste
Parameter Unit A1 A2 A3 A4
HW kg 2,47E-04 5,11E-06 1,74E-07 2,44E-06
NHW kg 5,98E+00 8,73E-01 1,03E-02 4,16E-01
RW kg INA* INA* INA* INA*
HW Hazardous waste disposed; NHW Non hazardous waste disposed; RW Radioactive waste disposed
Reading example: 9,0 E-03 = 9,0*10-3 = 0,009
*INA Indicator Not Assessed
End of life - Output flow
Parameter Unit A1 A2 A3 A4
CR kg 0,00E+00 0,00E+00 0,00E+00 0,00E+00
MR kg 0,00E+00 0,00E+00 0,00E+00 0,00E+00
MER kg 0,00E+00 0,00E+00 0,00E+00 0,00E+00
EEE MJ INA* INA* INA* INA*
ETE MJ INA* INA* INA* INA*
CR Components for reuse; MR Materials for recycling; MER Materials for energy recovery; EEE Exported electric energy; ETE Exported thermal
energy
Reading example: 9,0 E-03 = 9,0*10-3 = 0,009
*INA Indicator Not Assessed
Additional Norwegian requirements
Greenhouse gas emissions from the use of electricity in the manufacturing phase
National production mix from import, low voltage (production of transmission lines, in addition to direct emissions and losses in grid) of applied
electricity for the manufacturing process (A3).
Electricity mix Data source Amount Unit
El-mix, Norway (kWh) ecoinvent 3.4 31,04 g CO2-ekv/kWh
Dangerous substances
The product contains no substances given by the REACH Candidate list or the Norwegian priority list.
Indoor environment
Our furniture doesn't contain any substanses that effect indoor climate.
Additional environmental information
Bibliography
ISO 14025:2010 Environmental labels and declarations - Type III environmental declarations - Principles and procedures.
ISO 14044:2006 Environmental management - Life cycle assessment - Requirements and guidelines.
EN 15804:2012+A1:2013 Environmental product declaration - Core rules for the product category of construction products.
ISO 21930:2017 Sustainability in buildings and civil engineering works - Core rules for environmental product declarations of construction products.
ecoinvent v3, Allocation, cut-off by classification, Swiss Centre of Life Cycle Inventories.
Iversen et al., (2018) eEPD v3.0 - Background information for EPD generator system. LCA.no report number 04.18
Vold et al., (2019) EPD generator for Norsk Industri, Background information for industry application and LCA data, LCA.no report number 06.19.
NPCR Part A: Construction products and services. Ver. 1.0. April 2017, EPD-Norge.
NPCR 026 Part B for Furniture. Ver. 2.0 October 2018, EPD-Norge.
Program operator and publisher Phone: +47 97722020
The Norwegian EPD Foundation
Post Box 5250 Majorstuen, 0303 Oslo e-mail: post@epd-norge.no
0303 Oslo Norway web: www.epd-norge.no
Owner of the declaration Phone: +47 700 46 000
Fora Form AS Fax:
Mosfaltevegen e-mail: info@foraform.com
6154 Ørsta web: www.foraform.no
Author of the Life Cycle Assessment Phone: +47 916 50 916
LCA.no AS Fax:
Dokka 1C e-mail: post@lca.no
1671 Kråkerøy web: www.lca.no
Developer of EPD generator Phone: +47 916 50 916
LCA.no AS
Dokka 1C e-mail: post@lca.no
1671 Kråkerøy web: www.lca.no
ver1 2015
ENVIRONMENTAL PRODUCT DECLARATION
in accordance with ISO 14025, ISO 21930 and EN 15804
Owner of the declaration: Fora Form AS
Program operator: The Norwegian EPD Foundation
The Norwegian EPD Foundation
Publisher:
Declaration number: NEPD-2203-1001-EN
Registration number: NEPD-2203-1001-EN
ECO Platform reference number: -
Issue date: 26.05.2020
Valid to: 26.05.2025
Knekk stool
Fora Form AS
www.epd-norge.no
General information
Product: Owner of the declaration:
Knekk stool Fora Form AS
Contact person: Camilla Løseth
Phone: +47 700 46 000
e-mail: info@foraform.com
Program operator: Manufacturer:
The Norwegian EPD Foundation Fora Form AS
Pb. 5250 Majorstuen, 0303 Oslo
Phone: +47 97722020
e-mail: post@epd-norge.no
Declaration number: Place of production:
NEPD-2203-1001-EN Mosflatevegen
6154 Ørsta
N
ECO Platform reference number: Management system:
NS-EN ISO 14001: 2015 No. 800406. NS-EN ISO 9001: 2015 No.
901268. NS-EN ISO 45001: 2018 No 907167.
This declaration is based on Product Category Rules: Organisation no:
CEN Standard EN 15804:2012+A1:2013 serves as core PCR 986 581 421
PCR fot furniture NPCR 021 , Norwegian EPD Foundation
Statement of liability: Issue date: 26.05.2020
The owner of the declaration shall be liable for the underlying
information and evidence. EPD Norway shall not be liable with Valid to: 26.05.2025
respect to manufacturer information, life cycle assessment data and
evidences.
Declared unit: Year of study:
1 Pcs Knekk stool 2020
Declared unit with option: Comparability:
A1,A2,A3,A4 EPDs from programmes other than the Norwegian EPD Foundation
may not be comparable
Functional unit: Author of the Life Cycle Assessment:
The declaration is developed using eEPD v3.0 from LCA.no
Approval:
Company specific data are:
Collected/registered by: Kåre Sætre
Internal verification by: Camilla Løseth
Verification: Approved:
Independent verification of data, other environmental information and
the declaration according to ISO14025:2010, § 8.1.3 and § 8.1.4
Third party verifier:
Sign Sign
Seniorforsker Erik Svanes
(Independent verifier approved by EPD Norway)
Key environmental indicators Unit Cradle to gate A1 - A3
Global warming kg CO2 eqv 3,34
Total energy use MJ 134,25
Amount of recycled materials % 16,60
Product
Market: Technical data:
Dimensions: W: 46 cm H: 66 cm D: 53 cm SH: 66 cm
Worldwide
Weight : 5 kg ( packaging exluded )
Product description:
Reference service life, product
Interaction and function meet Nordic minimalism. The horizontal part of
the seat provides for reflection and relaxation. The askew part of the seat
gives direction for active interaction and support new and innovative
Reference service life, building
processes.
“Knekk” is a student work by Jon Fauske designed to capture Fora Form
values in a young and surprising fashion.
The modern designed solid wood stool is stackable with brass details.
Natural oak. Stackable. Brass cover on footrest.
Product specification
Recycled share in Recycled share in
Materials kg %
material (kg) material (%)
Metal - Brass 0,20 4,27 0,00 0,00
Plastic - Polyoxymethylene (POM) 0,01 0,13 0,00 50,00
Wood - Solid oak 4,40 93,90 0,00 0,00
Paint, water-based 0,40 1,71 0,00 0,00
Recycled share in Recycled share in
Packaging kg
material (kg) material (%)
Packaging - Cardboard 1,50 1,14 76,30
LCA: Calculation rules
Declared unit: Allocation:
The allocation is made in accordance with the provisions of EN 15804.
1 Pcs Knekk stool
Effects of primary production of recycled materials is allocated to the
Cut-off criteria: main product in which the material was used. The recycling process and
All major raw materials and all the essential energy is included. The transportation of the material is allocated to this analysis.
production processes for raw materials and energy flows with very small
amounts (less than 1%) are not included. These cut-off criteria do not
apply for hazardous materials and substances.
Data quality:
Specific data for the product composition are provided by the manufacturer. They represent the production of the declared product and were collected
for EPD development in the year of study. Background data is based on registered EPDs according to EN 15804, Ostfold Research databases,
ecoinvent and other LCA databases. The data quality of the raw materials in A1 is presented in the table below.
Materials Source Data quality Year
Plastic - Polyoxymethylene (POM) ecoinvent 3.4 Database 2015
Metal - Brass ecoinvent 3.4 Database 2017
Metal - Steel ecoinvent 3.4 Database 2017
Packaging - Cardboard ecoinvent 3.4 Database 2017
Paint, water-based ecoinvent 3.4 Database 2017
Plastics ecoinvent 3.4 Database 2017
Wood - Solid oak ecoinvent 3.4 Database 2017
System boundary:
Additional technical information:
The following information describe the scenarios in the different modules of the EPD.
The following information describe the scenarios in the different modules of the EPD.
Transport from production place to user (A4)
Capacity
Fuel/Energy
Type utilisation (incl. Type of vehicle Distance km Unit Value (l/t)
consumption
return) %
Truck, over 32
Truck 55,0 % 500 0,022823 l/tkm 11,41
tonnes, EURO 5
Railway l/tkm
Boat l/tkm
Other Transportation l/tkm
LCA: Results
System boundaries (X=included, MND=module not declared, MNR=module not relevant)
Construction Beyond the
Product stage installation User stage End of life stage . system
stage bondaries
A1 A2 A3 A4 A5 B1 B2 B3 B4 B5 B6 B7 C1 C2 C3 C4 . D
X X X X MND MND MND MND MND MND MNR MND MND MND MND MND . MND
Environmental impact
Parameter Unit A1 A2 A3 A4
GWP kg CO 2 -eq 3,34E+00 5,94E-01 7,76E-03 2,83E-01
ODP kg CFC11 -eq 2,86E-07 1,16E-07 7,34E-10 5,53E-08
POCP kg C 2H 4-eq 3,02E-03 9,61E-05 1,74E-06 4,58E-05
AP kg SO 2 -eq 6,61E-02 1,93E-03 3,62E-05 9,22E-04
EP kg PO3- -eq 1,76E-02 3,24E-04 8,73E-06 1,55E-04
4
ADPM kg Sb -eq 6,74E-04 1,34E-06 1,27E-07 6,40E-07
ADPE MJ 3,84E+01 9,33E+00 7,87E-02 4,45E+00
GWP Global warming potential; ODP Depletion potential of the stratospheric ozone layer; POCP Formation potential of tropospheric photochemical
oxidants; AP Acidification potential of land and water; EP Eutrophication potential; ADPM Abiotic depletion potential for non fossil resources; ADPE
Abiotic depletion potential for fossil resources
Reading example: 9,0 E-03 = 9,0*10-3 = 0,009
*INA Indicator Not Assessed
waR slairetam tropsnarT
gnirutcafunaM
tropsnarT ylbmessA esU ecnanetniaM riapeR tnemecalpeR
tnemhsibrufeR
lanoitarepO ygrene esu lanoitarepO esu retaw -eD noitcurtsnoc noitilomed tropsnarT etsaW gnissecorp lasopsiD
-yrevoceR-esueR
-gnilcyceR laitnetop
NEPD-2203-1001-EN Knekk stool 6 / 8
Resource use
Parameter Unit A1 A2 A3 A4
RPEE MJ 9,09E+01 1,69E-01 1,02E+00 8,04E-02
RPEM MJ 5,83E+01 0,00E+00 0,00E+00 0,00E+00
TPE MJ 1,49E+02 1,69E-01 1,02E+00 8,04E-02
NRPE MJ 4,33E+01 9,62E+00 1,35E-01 4,59E+00
NRPM MJ 1,11E-01 0,00E+00 0,00E+00 0,00E+00
TRPE MJ 4,34E+01 9,62E+00 1,35E-01 4,59E+00
SM kg 1,15E+00 0,00E+00 0,00E+00 0,00E+00
RSF MJ 0,00E+00 0,00E+00 1,77E-04 0,00E+00
NRSF MJ 0,00E+00 0,00E+00 0,00E+00 0,00E+00
W m3 6,72E-02 2,27E-03 5,65E-05 1,08E-03
RPEE Renewable primary energy resources used as energy carrier; RPEM Renewable primary energy resources used as raw materials; TPE Total use
of renewable primary energy resources; NRPE Non renewable primary energy resources used as energy carrier; NRPM Non renewable primary energy
resources used as materials; TRPE Total use of non renewable primary energy resources; SM Use of secondary materials; RSF Use of renewable
secondary fuels; NRSF Use of non renewable secondary fuels; W Use of net fresh water
Reading example: 9,0 E-03 = 9,0*10-3 = 0,009
*INA Indicator Not Assessed
End of life - Waste
Parameter Unit A1 A2 A3 A4
HW kg 2,47E-04 5,11E-06 1,74E-07 2,44E-06
NHW kg 5,98E+00 8,73E-01 1,03E-02 4,16E-01
RW kg INA* INA* INA* INA*
HW Hazardous waste disposed; NHW Non hazardous waste disposed; RW Radioactive waste disposed
Reading example: 9,0 E-03 = 9,0*10-3 = 0,009
*INA Indicator Not Assessed
End of life - Output flow
Parameter Unit A1 A2 A3 A4
CR kg 0,00E+00 0,00E+00 0,00E+00 0,00E+00
MR kg 0,00E+00 0,00E+00 0,00E+00 0,00E+00
MER kg 0,00E+00 0,00E+00 0,00E+00 0,00E+00
EEE MJ INA* INA* INA* INA*
ETE MJ INA* INA* INA* INA*
CR Components for reuse; MR Materials for recycling; MER Materials for energy recovery; EEE Exported electric energy; ETE Exported thermal
energy
Reading example: 9,0 E-03 = 9,0*10-3 = 0,009
*INA Indicator Not Assessed
Additional Norwegian requirements
Greenhouse gas emissions from the use of electricity in the manufacturing phase
National production mix from import, low voltage (production of transmission lines, in addition to direct emissions and losses in grid) of applied
electricity for the manufacturing process (A3).
Electricity mix Data source Amount Unit
El-mix, Norway (kWh) ecoinvent 3.4 31,04 g CO2-ekv/kWh
Dangerous substances
The product contains no substances given by the REACH Candidate list or the Norwegian priority list.
Indoor environment
Our furniture doesn't contain any substanses that effect indoor climate.
Additional environmental information
Bibliography
ISO 14025:2010 Environmental labels and declarations - Type III environmental declarations - Principles and procedures.
ISO 14044:2006 Environmental management - Life cycle assessment - Requirements and guidelines.
EN 15804:2012+A1:2013 Environmental product declaration - Core rules for the product category of construction products.
ISO 21930:2017 Sustainability in buildings and civil engineering works - Core rules for environmental product declarations of construction products.
ecoinvent v3, Allocation, cut-off by classification, Swiss Centre of Life Cycle Inventories.
Iversen et al., (2018) eEPD v3.0 - Background information for EPD generator system. LCA.no report number 04.18
Vold et al., (2019) EPD generator for Norsk Industri, Background information for industry application and LCA data, LCA.no report number 06.19.
NPCR Part A: Construction products and services. Ver. 1.0. April 2017, EPD-Norge.
NPCR 026 Part B for Furniture. Ver. 2.0 October 2018, EPD-Norge.
Program operator and publisher Phone: +47 97722020
The Norwegian EPD Foundation
Post Box 5250 Majorstuen, 0303 Oslo e-mail: post@epd-norge.no
0303 Oslo Norway web: www.epd-norge.no
Owner of the declaration Phone: +47 700 46 000
Fora Form AS Fax:
Mosfaltevegen e-mail: info@foraform.com
6154 Ørsta web: www.foraform.no
Author of the Life Cycle Assessment Phone: +47 916 50 916
LCA.no AS Fax:
Dokka 1C e-mail: post@lca.no
1671 Kråkerøy web: www.lca.no
Developer of EPD generator Phone: +47 916 50 916
LCA.no AS
Dokka 1C e-mail: post@lca.no
1671 Kråkerøy web: www.lca.no
ver1 2015
ENVIRONMENTAL PRODUCT DECLARATION
in accordance with ISO 14025, ISO 21930 and EN 15804
Owner of the declaration: Fora Form AS
Program operator: The Norwegian EPD Foundation
The Norwegian EPD Foundation
Publisher:
Declaration number: NEPD-2203-1001-EN
Registration number: NEPD-2203-1001-EN
ECO Platform reference number: -
Issue date: 26.05.2020
Valid to: 26.05.2025
Knekk stool
Fora Form AS
www.epd-norge.no
General information
Product: Owner of the declaration:
Knekk stool Fora Form AS
Contact person: Camilla Løseth
Phone: +47 700 46 000
e-mail: info@foraform.com
Program operator: Manufacturer:
The Norwegian EPD Foundation Fora Form AS
Pb. 5250 Majorstuen, 0303 Oslo
Phone: +47 97722020
e-mail: post@epd-norge.no
Declaration number: Place of production:
NEPD-2203-1001-EN Mosflatevegen
6154 Ørsta
N
ECO Platform reference number: Management system:
NS-EN ISO 14001: 2015 No. 800406. NS-EN ISO 9001: 2015 No.
901268. NS-EN ISO 45001: 2018 No 907167.
This declaration is based on Product Category Rules: Organisation no:
CEN Standard EN 15804:2012+A1:2013 serves as core PCR 986 581 421
PCR fot furniture NPCR 021 , Norwegian EPD Foundation
Statement of liability: Issue date: 26.05.2020
The owner of the declaration shall be liable for the underlying
information and evidence. EPD Norway shall not be liable with Valid to: 26.05.2025
respect to manufacturer information, life cycle assessment data and
evidences.
Declared unit: Year of study:
1 Pcs Knekk stool 2020
Declared unit with option: Comparability:
A1,A2,A3,A4 EPDs from programmes other than the Norwegian EPD Foundation
may not be comparable
Functional unit: Author of the Life Cycle Assessment:
The declaration is developed using eEPD v3.0 from LCA.no
Approval:
Company specific data are:
Collected/registered by: Kåre Sætre
Internal verification by: Camilla Løseth
Verification: Approved:
Independent verification of data, other environmental information and
the declaration according to ISO14025:2010, § 8.1.3 and § 8.1.4
Third party verifier:
Sign Sign
Seniorforsker Erik Svanes
(Independent verifier approved by EPD Norway)
Key environmental indicators Unit Cradle to gate A1 - A3
Global warming kg CO2 eqv 3,34
Total energy use MJ 134,25
Amount of recycled materials % 16,60
Product
Market: Technical data:
Dimensions: W: 46 cm H: 66 cm D: 53 cm SH: 66 cm
Worldwide
Weight : 5 kg ( packaging exluded )
Product description:
Reference service life, product
Interaction and function meet Nordic minimalism. The horizontal part of
the seat provides for reflection and relaxation. The askew part of the seat
gives direction for active interaction and support new and innovative
Reference service life, building
processes.
“Knekk” is a student work by Jon Fauske designed to capture Fora Form
values in a young and surprising fashion.
The modern designed solid wood stool is stackable with brass details.
Natural oak. Stackable. Brass cover on footrest.
Product specification
Recycled share in Recycled share in
Materials kg %
material (kg) material (%)
Metal - Brass 0,20 4,27 0,00 0,00
Plastic - Polyoxymethylene (POM) 0,01 0,13 0,00 50,00
Wood - Solid oak 4,40 93,90 0,00 0,00
Paint, water-based 0,40 1,71 0,00 0,00
Recycled share in Recycled share in
Packaging kg
material (kg) material (%)
Packaging - Cardboard 1,50 1,14 76,30
LCA: Calculation rules
Declared unit: Allocation:
The allocation is made in accordance with the provisions of EN 15804.
1 Pcs Knekk stool
Effects of primary production of recycled materials is allocated to the
Cut-off criteria: main product in which the material was used. The recycling process and
All major raw materials and all the essential energy is included. The transportation of the material is allocated to this analysis.
production processes for raw materials and energy flows with very small
amounts (less than 1%) are not included. These cut-off criteria do not
apply for hazardous materials and substances.
Data quality:
Specific data for the product composition are provided by the manufacturer. They represent the production of the declared product and were collected
for EPD development in the year of study. Background data is based on registered EPDs according to EN 15804, Ostfold Research databases,
ecoinvent and other LCA databases. The data quality of the raw materials in A1 is presented in the table below.
Materials Source Data quality Year
Plastic - Polyoxymethylene (POM) ecoinvent 3.4 Database 2015
Metal - Brass ecoinvent 3.4 Database 2017
Metal - Steel ecoinvent 3.4 Database 2017
Packaging - Cardboard ecoinvent 3.4 Database 2017
Paint, water-based ecoinvent 3.4 Database 2017
Plastics ecoinvent 3.4 Database 2017
Wood - Solid oak ecoinvent 3.4 Database 2017
System boundary:
Additional technical information:
The following information describe the scenarios in the different modules of the EPD.
The following information describe the scenarios in the different modules of the EPD.
Transport from production place to user (A4)
Capacity
Fuel/Energy
Type utilisation (incl. Type of vehicle Distance km Unit Value (l/t)
consumption
return) %
Truck, over 32
Truck 55,0 % 500 0,022823 l/tkm 11,41
tonnes, EURO 5
Railway l/tkm
Boat l/tkm
Other Transportation l/tkm
LCA: Results
System boundaries (X=included, MND=module not declared, MNR=module not relevant)
Construction Beyond the
Product stage installation User stage End of life stage . system
stage bondaries
A1 A2 A3 A4 A5 B1 B2 B3 B4 B5 B6 B7 C1 C2 C3 C4 . D
X X X X MND MND MND MND MND MND MNR MND MND MND MND MND . MND
Environmental impact
Parameter Unit A1 A2 A3 A4
GWP kg CO 2 -eq 3,34E+00 5,94E-01 7,76E-03 2,83E-01
ODP kg CFC11 -eq 2,86E-07 1,16E-07 7,34E-10 5,53E-08
POCP kg C 2H 4-eq 3,02E-03 9,61E-05 1,74E-06 4,58E-05
AP kg SO 2 -eq 6,61E-02 1,93E-03 3,62E-05 9,22E-04
EP kg PO3- -eq 1,76E-02 3,24E-04 8,73E-06 1,55E-04
4
ADPM kg Sb -eq 6,74E-04 1,34E-06 1,27E-07 6,40E-07
ADPE MJ 3,84E+01 9,33E+00 7,87E-02 4,45E+00
GWP Global warming potential; ODP Depletion potential of the stratospheric ozone layer; POCP Formation potential of tropospheric photochemical
oxidants; AP Acidification potential of land and water; EP Eutrophication potential; ADPM Abiotic depletion potential for non fossil resources; ADPE
Abiotic depletion potential for fossil resources
Reading example: 9,0 E-03 = 9,0*10-3 = 0,009
*INA Indicator Not Assessed
waR slairetam tropsnarT
gnirutcafunaM
tropsnarT ylbmessA esU ecnanetniaM riapeR tnemecalpeR
tnemhsibrufeR
lanoitarepO ygrene esu lanoitarepO esu retaw -eD noitcurtsnoc noitilomed tropsnarT etsaW gnissecorp lasopsiD
-yrevoceR-esueR
-gnilcyceR laitnetop
Resource use
Parameter Unit A1 A2 A3 A4
RPEE MJ 9,09E+01 1,69E-01 1,02E+00 8,04E-02
RPEM MJ 5,83E+01 0,00E+00 0,00E+00 0,00E+00
TPE MJ 1,49E+02 1,69E-01 1,02E+00 8,04E-02
NRPE MJ 4,33E+01 9,62E+00 1,35E-01 4,59E+00
NRPM MJ 1,11E-01 0,00E+00 0,00E+00 0,00E+00
TRPE MJ 4,34E+01 9,62E+00 1,35E-01 4,59E+00
SM kg 1,15E+00 0,00E+00 0,00E+00 0,00E+00
RSF MJ 0,00E+00 0,00E+00 1,77E-04 0,00E+00
NRSF MJ 0,00E+00 0,00E+00 0,00E+00 0,00E+00
W m3 6,72E-02 2,27E-03 5,65E-05 1,08E-03
RPEE Renewable primary energy resources used as energy carrier; RPEM Renewable primary energy resources used as raw materials; TPE Total use
of renewable primary energy resources; NRPE Non renewable primary energy resources used as energy carrier; NRPM Non renewable primary energy
resources used as materials; TRPE Total use of non renewable primary energy resources; SM Use of secondary materials; RSF Use of renewable
secondary fuels; NRSF Use of non renewable secondary fuels; W Use of net fresh water
Reading example: 9,0 E-03 = 9,0*10-3 = 0,009
*INA Indicator Not Assessed
End of life - Waste
Parameter Unit A1 A2 A3 A4
HW kg 2,47E-04 5,11E-06 1,74E-07 2,44E-06
NHW kg 5,98E+00 8,73E-01 1,03E-02 4,16E-01
RW kg INA* INA* INA* INA*
HW Hazardous waste disposed; NHW Non hazardous waste disposed; RW Radioactive waste disposed
Reading example: 9,0 E-03 = 9,0*10-3 = 0,009
*INA Indicator Not Assessed
End of life - Output flow
Parameter Unit A1 A2 A3 A4
CR kg 0,00E+00 0,00E+00 0,00E+00 0,00E+00
MR kg 0,00E+00 0,00E+00 0,00E+00 0,00E+00
MER kg 0,00E+00 0,00E+00 0,00E+00 0,00E+00
EEE MJ INA* INA* INA* INA*
ETE MJ INA* INA* INA* INA*
CR Components for reuse; MR Materials for recycling; MER Materials for energy recovery; EEE Exported electric energy; ETE Exported thermal
energy
Reading example: 9,0 E-03 = 9,0*10-3 = 0,009
*INA Indicator Not Assessed
NEPD-2203-1001-EN Knekk stool 7 / 8
Additional Norwegian requirements
Greenhouse gas emissions from the use of electricity in the manufacturing phase
National production mix from import, low voltage (production of transmission lines, in addition to direct emissions and losses in grid) of applied
electricity for the manufacturing process (A3).
Electricity mix Data source Amount Unit
El-mix, Norway (kWh) ecoinvent 3.4 31,04 g CO2-ekv/kWh
Dangerous substances
The product contains no substances given by the REACH Candidate list or the Norwegian priority list.
Indoor environment
Our furniture doesn't contain any substanses that effect indoor climate.
Additional environmental information
Bibliography
ISO 14025:2010 Environmental labels and declarations - Type III environmental declarations - Principles and procedures.
ISO 14044:2006 Environmental management - Life cycle assessment - Requirements and guidelines.
EN 15804:2012+A1:2013 Environmental product declaration - Core rules for the product category of construction products.
ISO 21930:2017 Sustainability in buildings and civil engineering works - Core rules for environmental product declarations of construction products.
ecoinvent v3, Allocation, cut-off by classification, Swiss Centre of Life Cycle Inventories.
Iversen et al., (2018) eEPD v3.0 - Background information for EPD generator system. LCA.no report number 04.18
Vold et al., (2019) EPD generator for Norsk Industri, Background information for industry application and LCA data, LCA.no report number 06.19.
NPCR Part A: Construction products and services. Ver. 1.0. April 2017, EPD-Norge.
NPCR 026 Part B for Furniture. Ver. 2.0 October 2018, EPD-Norge.
Program operator and publisher Phone: +47 97722020
The Norwegian EPD Foundation
Post Box 5250 Majorstuen, 0303 Oslo e-mail: post@epd-norge.no
0303 Oslo Norway web: www.epd-norge.no
Owner of the declaration Phone: +47 700 46 000
Fora Form AS Fax:
Mosfaltevegen e-mail: info@foraform.com
6154 Ørsta web: www.foraform.no
Author of the Life Cycle Assessment Phone: +47 916 50 916
LCA.no AS Fax:
Dokka 1C e-mail: post@lca.no
1671 Kråkerøy web: www.lca.no
Developer of EPD generator Phone: +47 916 50 916
LCA.no AS
Dokka 1C e-mail: post@lca.no
1671 Kråkerøy web: www.lca.no
ver1 2015
ENVIRONMENTAL PRODUCT DECLARATION
in accordance with ISO 14025, ISO 21930 and EN 15804
Owner of the declaration: Fora Form AS
Program operator: The Norwegian EPD Foundation
The Norwegian EPD Foundation
Publisher:
Declaration number: NEPD-2203-1001-EN
Registration number: NEPD-2203-1001-EN
ECO Platform reference number: -
Issue date: 26.05.2020
Valid to: 26.05.2025
Knekk stool
Fora Form AS
www.epd-norge.no
General information
Product: Owner of the declaration:
Knekk stool Fora Form AS
Contact person: Camilla Løseth
Phone: +47 700 46 000
e-mail: info@foraform.com
Program operator: Manufacturer:
The Norwegian EPD Foundation Fora Form AS
Pb. 5250 Majorstuen, 0303 Oslo
Phone: +47 97722020
e-mail: post@epd-norge.no
Declaration number: Place of production:
NEPD-2203-1001-EN Mosflatevegen
6154 Ørsta
N
ECO Platform reference number: Management system:
NS-EN ISO 14001: 2015 No. 800406. NS-EN ISO 9001: 2015 No.
901268. NS-EN ISO 45001: 2018 No 907167.
This declaration is based on Product Category Rules: Organisation no:
CEN Standard EN 15804:2012+A1:2013 serves as core PCR 986 581 421
PCR fot furniture NPCR 021 , Norwegian EPD Foundation
Statement of liability: Issue date: 26.05.2020
The owner of the declaration shall be liable for the underlying
information and evidence. EPD Norway shall not be liable with Valid to: 26.05.2025
respect to manufacturer information, life cycle assessment data and
evidences.
Declared unit: Year of study:
1 Pcs Knekk stool 2020
Declared unit with option: Comparability:
A1,A2,A3,A4 EPDs from programmes other than the Norwegian EPD Foundation
may not be comparable
Functional unit: Author of the Life Cycle Assessment:
The declaration is developed using eEPD v3.0 from LCA.no
Approval:
Company specific data are:
Collected/registered by: Kåre Sætre
Internal verification by: Camilla Løseth
Verification: Approved:
Independent verification of data, other environmental information and
the declaration according to ISO14025:2010, § 8.1.3 and § 8.1.4
Third party verifier:
Sign Sign
Seniorforsker Erik Svanes
(Independent verifier approved by EPD Norway)
Key environmental indicators Unit Cradle to gate A1 - A3
Global warming kg CO2 eqv 3,34
Total energy use MJ 134,25
Amount of recycled materials % 16,60
Product
Market: Technical data:
Dimensions: W: 46 cm H: 66 cm D: 53 cm SH: 66 cm
Worldwide
Weight : 5 kg ( packaging exluded )
Product description:
Reference service life, product
Interaction and function meet Nordic minimalism. The horizontal part of
the seat provides for reflection and relaxation. The askew part of the seat
gives direction for active interaction and support new and innovative
Reference service life, building
processes.
“Knekk” is a student work by Jon Fauske designed to capture Fora Form
values in a young and surprising fashion.
The modern designed solid wood stool is stackable with brass details.
Natural oak. Stackable. Brass cover on footrest.
Product specification
Recycled share in Recycled share in
Materials kg %
material (kg) material (%)
Metal - Brass 0,20 4,27 0,00 0,00
Plastic - Polyoxymethylene (POM) 0,01 0,13 0,00 50,00
Wood - Solid oak 4,40 93,90 0,00 0,00
Paint, water-based 0,40 1,71 0,00 0,00
Recycled share in Recycled share in
Packaging kg
material (kg) material (%)
Packaging - Cardboard 1,50 1,14 76,30
LCA: Calculation rules
Declared unit: Allocation:
The allocation is made in accordance with the provisions of EN 15804.
1 Pcs Knekk stool
Effects of primary production of recycled materials is allocated to the
Cut-off criteria: main product in which the material was used. The recycling process and
All major raw materials and all the essential energy is included. The transportation of the material is allocated to this analysis.
production processes for raw materials and energy flows with very small
amounts (less than 1%) are not included. These cut-off criteria do not
apply for hazardous materials and substances.
Data quality:
Specific data for the product composition are provided by the manufacturer. They represent the production of the declared product and were collected
for EPD development in the year of study. Background data is based on registered EPDs according to EN 15804, Ostfold Research databases,
ecoinvent and other LCA databases. The data quality of the raw materials in A1 is presented in the table below.
Materials Source Data quality Year
Plastic - Polyoxymethylene (POM) ecoinvent 3.4 Database 2015
Metal - Brass ecoinvent 3.4 Database 2017
Metal - Steel ecoinvent 3.4 Database 2017
Packaging - Cardboard ecoinvent 3.4 Database 2017
Paint, water-based ecoinvent 3.4 Database 2017
Plastics ecoinvent 3.4 Database 2017
Wood - Solid oak ecoinvent 3.4 Database 2017
System boundary:
Additional technical information:
The following information describe the scenarios in the different modules of the EPD.
The following information describe the scenarios in the different modules of the EPD.
Transport from production place to user (A4)
Capacity
Fuel/Energy
Type utilisation (incl. Type of vehicle Distance km Unit Value (l/t)
consumption
return) %
Truck, over 32
Truck 55,0 % 500 0,022823 l/tkm 11,41
tonnes, EURO 5
Railway l/tkm
Boat l/tkm
Other Transportation l/tkm
LCA: Results
System boundaries (X=included, MND=module not declared, MNR=module not relevant)
Construction Beyond the
Product stage installation User stage End of life stage . system
stage bondaries
A1 A2 A3 A4 A5 B1 B2 B3 B4 B5 B6 B7 C1 C2 C3 C4 . D
X X X X MND MND MND MND MND MND MNR MND MND MND MND MND . MND
Environmental impact
Parameter Unit A1 A2 A3 A4
GWP kg CO 2 -eq 3,34E+00 5,94E-01 7,76E-03 2,83E-01
ODP kg CFC11 -eq 2,86E-07 1,16E-07 7,34E-10 5,53E-08
POCP kg C 2H 4-eq 3,02E-03 9,61E-05 1,74E-06 4,58E-05
AP kg SO 2 -eq 6,61E-02 1,93E-03 3,62E-05 9,22E-04
EP kg PO3- -eq 1,76E-02 3,24E-04 8,73E-06 1,55E-04
4
ADPM kg Sb -eq 6,74E-04 1,34E-06 1,27E-07 6,40E-07
ADPE MJ 3,84E+01 9,33E+00 7,87E-02 4,45E+00
GWP Global warming potential; ODP Depletion potential of the stratospheric ozone layer; POCP Formation potential of tropospheric photochemical
oxidants; AP Acidification potential of land and water; EP Eutrophication potential; ADPM Abiotic depletion potential for non fossil resources; ADPE
Abiotic depletion potential for fossil resources
Reading example: 9,0 E-03 = 9,0*10-3 = 0,009
*INA Indicator Not Assessed
waR slairetam tropsnarT
gnirutcafunaM
tropsnarT ylbmessA esU ecnanetniaM riapeR tnemecalpeR
tnemhsibrufeR
lanoitarepO ygrene esu lanoitarepO esu retaw -eD noitcurtsnoc noitilomed tropsnarT etsaW gnissecorp lasopsiD
-yrevoceR-esueR
-gnilcyceR laitnetop
Resource use
Parameter Unit A1 A2 A3 A4
RPEE MJ 9,09E+01 1,69E-01 1,02E+00 8,04E-02
RPEM MJ 5,83E+01 0,00E+00 0,00E+00 0,00E+00
TPE MJ 1,49E+02 1,69E-01 1,02E+00 8,04E-02
NRPE MJ 4,33E+01 9,62E+00 1,35E-01 4,59E+00
NRPM MJ 1,11E-01 0,00E+00 0,00E+00 0,00E+00
TRPE MJ 4,34E+01 9,62E+00 1,35E-01 4,59E+00
SM kg 1,15E+00 0,00E+00 0,00E+00 0,00E+00
RSF MJ 0,00E+00 0,00E+00 1,77E-04 0,00E+00
NRSF MJ 0,00E+00 0,00E+00 0,00E+00 0,00E+00
W m3 6,72E-02 2,27E-03 5,65E-05 1,08E-03
RPEE Renewable primary energy resources used as energy carrier; RPEM Renewable primary energy resources used as raw materials; TPE Total use
of renewable primary energy resources; NRPE Non renewable primary energy resources used as energy carrier; NRPM Non renewable primary energy
resources used as materials; TRPE Total use of non renewable primary energy resources; SM Use of secondary materials; RSF Use of renewable
secondary fuels; NRSF Use of non renewable secondary fuels; W Use of net fresh water
Reading example: 9,0 E-03 = 9,0*10-3 = 0,009
*INA Indicator Not Assessed
End of life - Waste
Parameter Unit A1 A2 A3 A4
HW kg 2,47E-04 5,11E-06 1,74E-07 2,44E-06
NHW kg 5,98E+00 8,73E-01 1,03E-02 4,16E-01
RW kg INA* INA* INA* INA*
HW Hazardous waste disposed; NHW Non hazardous waste disposed; RW Radioactive waste disposed
Reading example: 9,0 E-03 = 9,0*10-3 = 0,009
*INA Indicator Not Assessed
End of life - Output flow
Parameter Unit A1 A2 A3 A4
CR kg 0,00E+00 0,00E+00 0,00E+00 0,00E+00
MR kg 0,00E+00 0,00E+00 0,00E+00 0,00E+00
MER kg 0,00E+00 0,00E+00 0,00E+00 0,00E+00
EEE MJ INA* INA* INA* INA*
ETE MJ INA* INA* INA* INA*
CR Components for reuse; MR Materials for recycling; MER Materials for energy recovery; EEE Exported electric energy; ETE Exported thermal
energy
Reading example: 9,0 E-03 = 9,0*10-3 = 0,009
*INA Indicator Not Assessed
Additional Norwegian requirements
Greenhouse gas emissions from the use of electricity in the manufacturing phase
National production mix from import, low voltage (production of transmission lines, in addition to direct emissions and losses in grid) of applied
electricity for the manufacturing process (A3).
Electricity mix Data source Amount Unit
El-mix, Norway (kWh) ecoinvent 3.4 31,04 g CO2-ekv/kWh
Dangerous substances
The product contains no substances given by the REACH Candidate list or the Norwegian priority list.
Indoor environment
Our furniture doesn't contain any substanses that effect indoor climate.
Additional environmental information
Bibliography
ISO 14025:2010 Environmental labels and declarations - Type III environmental declarations - Principles and procedures.
ISO 14044:2006 Environmental management - Life cycle assessment - Requirements and guidelines.
EN 15804:2012+A1:2013 Environmental product declaration - Core rules for the product category of construction products.
ISO 21930:2017 Sustainability in buildings and civil engineering works - Core rules for environmental product declarations of construction products.
ecoinvent v3, Allocation, cut-off by classification, Swiss Centre of Life Cycle Inventories.
Iversen et al., (2018) eEPD v3.0 - Background information for EPD generator system. LCA.no report number 04.18
Vold et al., (2019) EPD generator for Norsk Industri, Background information for industry application and LCA data, LCA.no report number 06.19.
NPCR Part A: Construction products and services. Ver. 1.0. April 2017, EPD-Norge.
NPCR 026 Part B for Furniture. Ver. 2.0 October 2018, EPD-Norge.
Program operator and publisher Phone: +47 97722020
The Norwegian EPD Foundation
Post Box 5250 Majorstuen, 0303 Oslo e-mail: post@epd-norge.no
0303 Oslo Norway web: www.epd-norge.no
Owner of the declaration Phone: +47 700 46 000
Fora Form AS Fax:
Mosfaltevegen e-mail: info@foraform.com
6154 Ørsta web: www.foraform.no
Author of the Life Cycle Assessment Phone: +47 916 50 916
LCA.no AS Fax:
Dokka 1C e-mail: post@lca.no
1671 Kråkerøy web: www.lca.no
Developer of EPD generator Phone: +47 916 50 916
LCA.no AS
Dokka 1C e-mail: post@lca.no
1671 Kråkerøy web: www.lca.no
NEPD-2203-1001-EN Knekk stool 8 / 8
