Environmental product declaration
in accordance with ISO 14025 and EN 15804+A2
ROCKWOOL® Soundbatts for the Finnish market (R=1)
Owner of the declaration: Program operator:
ROCKWOOL Nordics The Norwegian EPD Foundation
Product: Declaration number:
ROCKWOOL® Soundbatts for the Finnish market (R=1) NEPD-5575-4874-EN
Declared unit: Registration number:
1 m2 NEPD-5575-4874-EN
This declaration is based on Product Category Rules: Issue date:
CEN Standard EN 15804:2012+A2:2019 serves as core 13.12.2023
PCR. NPCR Part A Construction products and services.
The Norwegian EPD Foundation Valid to:
NPCR 012:2022 Part B for Thermal insulation products
13.12.2028
EPD Software:
LCA.no EPD generator ID: 161638
1 / 11
General information
Product Owner of the declaration:
ROCKWOOL® Soundbatts for the Finnish market (R=1) ROCKWOOL Nordics
Contact person: Christian J. Kofod
Phone: +45 4656 1616
e-mail: info@rockwool.com
Program operator: Manufacturer:
Post Box 5250 Majorstuen, 0303 Oslo, Norway ROCKWOOL Nordics
The Norwegian EPD Foundation Hovedgaden 501
Phone: +47 23 08 80 00 DK-2640 Hedehusene, Denmark
web: post@epd-norge.no
Declaration number: NEPD-5575-4874-EN Place of production:
ROCKWOOL factory Moss (Electrical melter)
Værlegata 56
1531 Moss, Norway
This declaration is based on Product Category Rules: Management system:
CEN Standard EN 15804:2012+A2:2019 serves as core PCR. NPCR ISO 14001, ISO 9001
Part A Construction products and services.
NPCR 012:2022 Part B for Thermal insulation products
Statement of liability: Organisation no:
The owner of the declaration shall be liable for the underlying CVR nr. 42391719
information and evidence. EPD Norway shall not be liable with respect
to manufacturer information, life cycle assessment data and
evidences.​
Declared unit: Issue date:
1 m2 ROCKWOOL® Soundbatts for the Finnish market (R=1) 13.12.2023
Declared unit with option: Valid to:
A1-A3,A4,A5,C1,C2,C3,C4,D 13.12.2028
Year of study:
2021
Functional unit: Comparability:
Functional Unit Comparability: EPD of construction products may not be comparable if they not
The specific product referred to in the declared unit has the following comply with EN 15804:2012+A2:2019 and seen in a building context.
specifications: thickness: 40 mm; density 29 kg/m³; weight: 1,2 kg.
General information on verification of EPD from EPD tools: Development and verification of EPD:
Independent verification of data, other environmental information The declaration is created using EPD tool lca.tools ver EPD2022.03,
and the declaration according to ISO 14025:2010, § 8.1.3 and § 8.1.4. developed by LCA.no. The EPD tool is integrated in the company's
Verification of each EPD is made according to EPD-Norway’s management system, and has been approved by EPD Norway.
guidelines for verification and approval requiring that tools are i)
integrated into the company's environmental management system, ii) Developer of EPD: Nora Amlie Jansrud
the procedures for use of the EPD tool are approved by EPD-Norway,
Reviewer of company-specific input data and EPD:​ Christian Julius
and iii) the process is reviewed annually by an independent third
Kofod
party verifier. See Appendix G of EPD-Norway's General Programme
Instructions for further information on EPD tools
Verification of EPD tool: Approved:
Independent third party verification of the EPD tool, background data
and test-EPD in accordance with EPDNorway's procedures and
guidelines for verification and approval of EPD tools.
Third party verifier:
Jane Anderson, Construction LCA Ltd
(no signature required)
2 / 11
Product
Product description:
This EPD documents the potential environmental impacts of 1 m² of ROCKWOOL® Soundbatts stone wool insulation with a thermal resistance
(R-value) equal to 1 m²K/W. The intended use of the EPD is to communicate quantified environmental impacts of construction products for
application in the assessment of the environmental performance of buildings.
Product specification
The average composition used for this EPD is calculated based on average factory consumption figures for raw materials. The raw materials are
mainly non-scarce stones, and resin binder.
Materials Value Unit
Stone wool > 95 %
Binder < 5 %
De-duster and water repellency oil < 0.5 %
Technical data:
For the products covered by this EPD, the performance data are in accordance with the declaration of performance with respect to its essential
characteristics according to EN 13162:2012+A1:2015, "Thermal insulation products for buildings – Factory made mineral wool (MW) products –
Specification".
-Thermal conductivity: 0.04 W/mK, reference standards: EN 12939 and EN 12667
-Fire class: A1, reference standard: EN 13501-1:2007+ A1:2009
A full overview of the technical specifications can be found on www.rockwool.fi
Thickness (mm) Density (kg/m³) R-value (K·m²/W) Weight (kg) Scaling factor
50 27 1.25 1.4 1.13
66 27 1.65 1.8 1.49
70 27 1.75 1.9 1.58
95 27 2.38 2.6 2.14
Market:
This EPD is intended for the Finnish market. The EPD can be used in other specific Nordics markets by adjusting the A4 module to reflect correct
transportation distance.
Reference service life, product
ROCKWOOL® stone wool thermal insulation products are extremely durable and provide effective performance for the lifetime of a building or
host structure, with no need to be replaced. The thermal, fire-resistance, and acoustic performance of ROCKWOOL® stone wool products, when
correctly installed, remains the same during 60 years reference service life or as long as the insulation is part of the building.
Reference service life, building or construction works
In this EPD, the reference service life of a building is set to 60 years.
LCA: Calculation rules
Declared unit:
1 m2 ROCKWOOL® Soundbatts for the Finnish market (R=1)
Cut-off criteria:
All major raw materials and all the essential energy are included. All hazardous materials and substances are considered in the inventory. Data sets
within the system boundary are complete and fulfil criteria for the exclusion of inputs and output criteria. All data, materials and energy
consumptions, have been specified according to the production data and have been considered within the inventory analysis.
Allocation:
The allocation is made in accordance with the provisions of EN 15804+A2. Production activities, electricity and energy consumption and waste
generation are allocated equally among all products from the production site through mass allocation.
Data quality:
All data represents the applicable geography, time and technology for the specific and generic data, generally assessed as good and very good.
Primary data are collected from the specific production sites, in the reference year 2021 and represent stabilized production. Generic data is from
GaBi database (version 2021) with GaBi Software version 10.0.1.92.
3 / 11
System boundaries (X=included, MND=module not declared, MNR=module not relevant)
Construction Beyond the system
Product stage Use stage End of life stage
installation stage boundaries
A1 A2 A3 A4 A5 B1 B2 B3 B4 B5 B6 B7 C1 C2 C3 C4 D
X X X X X MNR MNR MNR MNR MNR MNR MNR X X X X X
System boundary:
The LCA is performed as a ‘cradle-to-grave’ study, addressing all life cycle stages identified in the EN 15804+A2. All major raw materials, energy,
electricity use and waste are included for all life cycle modules, see flowchart below. Use stage B1-7 modules are considered but are not relevant, as
there are no activities and no significant environmental impact in the use stage.
waR slairetam tropsnarT gnirutcafunaM tropsnarT ylbmessA e​sU ecnanetniaM riapeR tnemecalpeR tnemhsibrufeR lanoitarepO ygrene esu lanoitarepO esu retaw -eD noitcurtsnoc noitilomed tropsnarT etsaW gnissecorp lasopsiD -yrevoceR-esueR laitnetop-gnilcyceR
4 / 11
LCA: Scenarios and additional technical information
The following information describe the scenarios in the different modules of the EPD.
The EPD is based on LCA inventory data from the producing factories. The reference flow is a weighted average based on the distribution of
production capacity
Transport from production place to assembly/user (A4)
The A4 distance is calculated as weighted average distance for the Finnish market
Assembly (A5)
In A5 the default installation is assumed to be manual, therefore no energy consumption or ancillary equipment is needed. The product waste
from installation is assumed to be 2% and according to the modularity principle of EN 15804+A2 its impacts are fully allocated to A5, following
same EoL scenario as in C. The A5 module includes also the corresponding end-of-life considerations for packaging (10 % landfill). The credits from
heat and electricity recovery from incineration or material recycling from module A5 (90% recycling and energy recovery) are attributed to module
D.
Use stage (B1, B2, B3, B4, B5, B6, B7)
There are no consumables and no maintenance (B2), repair (B3), replacements (B4) or refurbishments (B5) required during the use of
ROCKWOOL® thermal insulation products in standard conditions. They do not use energy (B6) or water (B7) during their operational life. No LCA:
Scenarios and additional technical information EPD for the best environmental decision 8 significant emissions to the indoor environment occur in
module (B1). Therefore, modules B1-B7 are not relevant for this EPD and will not be displayed in the tables below.
Benefits and loads beyond the system boundaries (D)
Benefits in module D are created from packaging materials treatment after installation and recycling potential of stone wool in the end of life.
Quantities of packaging materials include both recycled materials and materials sent for energy recovery. Recycling potential of net stone wool
material is considered here.
Capacity utilisation Value
Transport from production place to user (A4) Distance (km) Fuel/Energy Consumption Unit
(incl. return) % (Liter/tonne)
Container ship, 5,000 to 200,000 dwt payload
40,0 % 395 0,004 l/tkm 1,58
capacity, ocean going (kgkm)
Transport from Moss: Truck, Euro 6, 27t payload
30,0 % 840 0,019 l/tkm 15,96
(kgkm)
Assembly (A5) Unit Value
Auxiliary kg 0,00
Cardboard and paper packaging kg 0,00
Electricity consumption kWh 0,00
Material loss kg 0,02
Other energy carriers MJ 0,00
Plastic packaging kg 0,02
Water consumption m3 0,00
Wood packaging kg 0,05
Capacity utilisation Value
Transport to waste processing (C2) Distance (km) Fuel/Energy Consumption Unit
(incl. return) % (Liter/tonne)
Waste transport, Norway: Truck, Euro 6 (kgkm) 50,0 % 150 0,025 l/tkm 3,75
Waste processing (C3) Unit Value
Collected as mixed construction waste kg 1,20
Energy recovery kg 0,00
Sent for recycling kg 0,00
Sent for reuse kg 0,00
Disposal (C4) Unit Value
Hazardous waste disposed kg 0,00
Sent to landfill kg 1,20
Benefits and loads beyond the system
Unit Value
boundaries (D)
Energy recovered MJ 0,36
Packaging recycled kg 0,02
5 / 11
LCA: Results
The LCA results are presented below for the declared unit defined on page 2 of the EPD document.
Environmental impact
Indicator Unit A1-A3 A4 A5 C1 C2 C3 C4 D
GWP-total kg CO2 -eq 4,59E-01 1,36E-01 1,03E-01 0 3,73E-03 0,00E+00 1,82E-02 -4,37E-02
GWP-fossil kg CO2 -eq 5,39E-01 1,35E-01 2,28E-02 0 3,71E-03 0,00E+00 1,81E-02 -4,81E-02
GWP-biogenic kg CO2 -eq -7,93E-02 0,00E+00 8,00E-02 0 0,00E+00 0,00E+00 0,00E+00 4,40E-03
GWP-luluc kg CO2 -eq 2,65E-04 1,06E-03 1,97E-05 0 3,05E-05 0,00E+00 5,33E-05 -3,65E-06
ODP kg CFC11 -eq 3,89E-09 0,00E+00 1,70E-10 0 0,00E+00 0,00E+00 0,00E+00 0,00E+00
AP mol H+ -eq 5,72E-03 3,74E-04 1,44E-04 0 3,91E-06 0,00E+00 1,30E-04 -1,32E-04
EP-FreshWater kg P -eq 1,00E-05 3,84E-07 3,01E-07 0 1,10E-08 0,00E+00 3,05E-08 -1,32E-08
EP-Marine kg N -eq 7,05E-04 9,96E-05 2,47E-05 0 1,28E-06 0,00E+00 3,36E-05 -2,46E-05
EP-Terrestial mol N -eq 2,11E-02 1,13E-03 5,24E-04 0 1,54E-05 0,00E+00 3,68E-04 -2,69E-04
POCP kg NMVOC -eq 1,51E-03 2,82E-04 5,54E-05 0 3,42E-06 0,00E+00 1,02E-04 -8,09E-05
ADP-minerals&metals1 kg Sb -eq 2,32E-07 0,00E+00 5,83E-09 0 3,60E-10 0,00E+00 1,72E-09 -4,18E-09
ADP-fossil1 MJ 6,73E+00 1,80E+00 2,66E-01 0 4,96E-02 0,00E+00 2,41E-01 -1,24E+00
WDP1 m3 1,71E-01 1,13E-03 1,23E-02 0 3,24E-05 0,00E+00 1,94E-03 -1,84E-02
GWP-total = Global Warming Potential total; GWP-fossil = Global Warming Potential fossil fuels; GWP-biogenic = Global Warming Potential biogenic; GWP-luluc =
Global Warming Potential land use and land use change; ODP = Depletion potential of the stratospheric ozone layer; AP = Acidification potential, Accumulated
Exceedance; EP-freshwater = Eutrophication potential, fraction of nutrients reaching freshwater end compartment: EP-marine = Eutrophication potential, fraction of
nutrients reaching marine end compartment; EP-terrestrial = Eutrophication potential, Accumulated Exceedance; POCP = Formation potential of tropospheric ozone;
ADP-minerals&metals = Abiotic depletion potential for non-fossil resources; ADP-fossil = Abiotic depletion for fossil resources potential; WDP = Water (user)
deprivation potential, deprivation-weighted water consumption
Reading example: 9,0 E-03 = 9,0*10-3 = 0,009
1. The results of this environmental impact indicator shall be used with care as the uncertainties on these results are high or as there is limited experienced with the
indicator.
Remarks to environmental impacts
The main GWP contribution from the product life cycle is linked to the Product stage (A1-A3). This is primarily related to the materials delivered to
the factory gate and consumption of
energy.
The CO2 absorbed by the wood in the wooden pallets is represented by a negative GWPbiogenic.
The GWP-Biogenic, e.g. the carbon stored in the wooden pallets, is released during the construction stage phase (A5) where the wood is
presumed incinerated with energy recovery.
The benefits from energy recovery (a negative GWP) from incineration of packaging materials (wood pallets and plastic foils) is allocated to
Benefits & Loads beyond system (D).
Impacts linked to end of life stages (C1-C4) are primarily linked to transportation of stone wool to recycling or to landfill.
Melting virgin materials or re-melting returned ROCKWOOL stone wool are both similarly energy intensive processes. Increasing the recycling rate
for return wool, will therefore not lead to great variations in the overall GWP profile. However, increased recycling will be linked directly to
reduction of waste sent to landfill.
6 / 11
Additional environmental impact indicators
Indicator Unit A1-A3 A4 A5 C1 C2 C3 C4 D
PM Disease incidence 5,50E-08 5,27E-09 1,32E-09 0 0,00E+00 0,00E+00 1,61E-09 -1,73E-09
IRP2 kgBq U235 -eq 7,20E-03 3,11E-04 1,56E-03 0 8,60E-06 0,00E+00 2,65E-04 -2,16E-04
ETP-fw1 CTUe 2,16E+00 1,30E+00 1,03E-01 0 3,59E-02 0,00E+00 1,37E-01 -1,40E-02
HTP-c1 CTUh 8,56E-10 0,00E+00 2,00E-11 0 0,00E+00 0,00E+00 2,00E-11 -5,00E-12
HTP-nc1 CTUh 2,67E-09 1,01E-09 2,87E-10 0 0,00E+00 0,00E+00 2,23E-09 -1,50E-10
SQP1 dimensionless 1,55E+01 5,92E-01 3,35E-01 0 1,70E-02 0,00E+00 4,86E-02 -7,85E-01
PM = Particulate Matter emissions; IRP = Ionizing radiation – human health; ETP-fw = Eco toxicity – freshwater; HTP-c = Human toxicity – cancer effects; HTP-nc =
Human toxicity – non cancer effects; SQP = Potential Soil Quality Index (dimensionless)
Reading example: 9,0 E-03 = 9,0*10-3 = 0,009
1. The results of this environmental impact indicator shall be used with care as the uncertainties on these results are high or as there is limited experienced with the
indicator.
2. This impact category deals mainly with the eventual impact of low dose ionizing radiation on human health of the nuclear fuel cycle. It does not consider effects due
to possible nuclear accidents, occupational exposure nor due to radioactive waste disposal in underground facilities. Potential ionizing radiation from the soil, from
radon and from some construction materials is also not measured by this indicator.
7 / 11
Resource use
Indicator Unit A1-A3 A4 A5 C1 C2 C3 C4 D
PERE MJ 7,72E+00 9,64E-02 1,86E-01 0 2,77E-03 0,00E+00 3,24E-02 -1,78E-01
PERM MJ 2,86E-03 0,00E+00 -8,59E-05 0 0,00E+00 0,00E+00 0,00E+00 0,00E+00
PERT MJ 7,72E+00 9,64E-02 1,86E-01 0 2,77E-03 0,00E+00 3,24E-02 -1,78E-01
PENRE MJ 5,98E+00 1,80E+00 2,74E-01 0 4,97E-02 0,00E+00 2,41E-01 -1,24E+00
PENRM MJ 7,55E-01 0,00E+00 -2,26E-02 0 0,00E+00 0,00E+00 0,00E+00 0,00E+00
PENRT MJ 6,74E+00 1,80E+00 2,51E-01 0 4,97E-02 0,00E+00 2,41E-01 -1,24E+00
SM kg 0,00E+00 0,00E+00 0,00E+00 0 0,00E+00 0,00E+00 0,00E+00 0,00E+00
RSF MJ 0,00E+00 0,00E+00 0,00E+00 0 0,00E+00 0,00E+00 0,00E+00 0,00E+00
NRSF MJ 0,00E+00 0,00E+00 0,00E+00 0 0,00E+00 0,00E+00 0,00E+00 0,00E+00
FW m3 4,14E-03 1,10E-04 3,06E-04 0 3,17E-06 0,00E+00 5,94E-05 -5,93E-04
PERE = Use of renewable primary energy excluding renewable primary energy resources used as raw materials; PERM = Use of renewable primary energy resources used
as raw materials; PERT = Total use of renewable primary energy resources; PENRE = Use of non renewable primary energy excluding non-renewable primary energy
resources used as raw materials; PENRM = Use of non renewable primary energy resources used as raw materials; PENRT = Total use of non renewable primary energy
resources; SM = Use of secondary materials; RSF = Use of renewable secondary fuels; NRSF = Use of non-renewable secondary fuels; FW = Net use of fresh water
Reading example: 9,0 E-03 = 9,0*10-3 = 0,009
8 / 11
End of life - Waste
Indicator Unit A1-A3 A4 A5 C1 C2 C3 C4 D
HWD kg 2,68E-07 0,00E+00 5,42E-09 0 0,00E+00 0,00E+00 2,50E-11 -1,09E-10
NHWD kg 4,19E-02 2,64E-04 3,13E-02 0 7,38E-06 0,00E+00 1,20E+00 -1,32E-04
RWD kg 2,08E-05 2,18E-06 1,04E-05 0 6,01E-08 0,00E+00 2,52E-06 -1,66E-06
HWD = Hazardous waste disposed; NHWD = Non-hazardous waste disposed; RWD = Radioactive waste disposed
Reading example: 9,0 E-03 = 9,0*10-3 = 0,009
End of life - Output flow
Indicator Unit A1-A3 A4 A5 C1 C2 C3 C4 D
CRU kg 0,00E+00 0,00E+00 0,00E+00 0 0,00E+00 0,00E+00 0,00E+00 0,00E+00
MFR kg 0,00E+00 0,00E+00 5,89E-02 0 0,00E+00 0,00E+00 0,00E+00 0,00E+00
MER kg 0,00E+00 0,00E+00 3,47E-03 0 0,00E+00 0,00E+00 0,00E+00 0,00E+00
EEE MJ 0,00E+00 0,00E+00 9,02E-02 0 0,00E+00 0,00E+00 0,00E+00 0,00E+00
EET MJ 0,00E+00 0,00E+00 2,69E-01 0 0,00E+00 0,00E+00 0,00E+00 0,00E+00
CRU = Components for re-use; MFR = Materials for recycling; MER = Materials for energy recovery; EEE = Exported energy electrical; EET = Exported energy thermal
Reading example: 9,0 E-03 = 9,0*10-3 = 0,009
Biogenic Carbon Content
Indicator Unit At the factory gate
Biogenic carbon content in product kg C 0,00E+00
Biogenic carbon content in accompanying packaging kg C 2,28E-02
Note: 1 kg biogenic carbon is equivalent to 44/12 kg CO2.
9 / 11
Additional requirements
Greenhouse gas emissions from the use of electricity in the manufacturing phase
National production mix from import, low voltage (production of transmission lines, in addition to direct emissions and losses in grid) of applied
electricity for the manufacturing process (A3).
Electricity mix Data source Amount Unit
Electricity, hydropower, Norway (kWh) GaBi (version 2021) 14,00 g CO2-eq/kWh
Dangerous substances
The product contains no substances given by the REACH Candidate list.
Indoor environment
There are no legal requirements for indoor emissions of stone wool thermal insulation products.
Additional Environmental Information
Additional environmental impact indicators required in NPCR Part A for construction products
Indicator Unit A1-A3 A4 A5 C1 C2 C3 C4 D
GWPIOBC kg CO2 -eq 5,39E-01 1,37E-01 2,29E-02 0 3,74E-03 0,00E+00 1,82E-02 -4,81E-02
GWP-IOBC: Global warming potential calculated according to the principle of instantaneous oxidation. In order to increase the transparency of biogenic carbon
contribution to climate impact, the indicator GWP-IOBC is required as it declares climate impacts calculated according to the principle of instantaneous oxidation.
GWP-IOBC is also referred to as GWP-GHG in context to Swedish public procurement legislation.
10 / 11
Bibliography
ISO 14025:2010 - Environmental labels and declarations - Type III environmental declarations - Principles and procedures
ISO 14044:2006 - Environmental management - Life cycle assessment - Requirements and guidelines
EN 15804:2012+A2:2019 - Sustainability of construction works - Environmental product declaration - Core rules for the product category of
construction products
EN 12939:2000 - Thermal performance of building materials and products - Determination of thermal resistance by means of guarded hot plate
and heat flow meter methods - Thick products of high and medium thermal resistance
EN 12667:2001 - Thermal performance of building materials and products – determination of thermal resistance by means of guarded hot plate
and heat flow meter methods – Products of high and medium thermal resistance
EN 13501-1:2007+A1:2009 - Fire classification of construction products and building elements - Part 1: Classification using data from reaction to
fire tests
ISO 21930:2007 - Sustainability in building construction - Environmental declaration of building products
PCR - NPCR Part A Construction products and services
PCR - NPCR 012:2022 version 2.0. Part B for Thermal insulation products
Larisa Xanthopoulou - Background LCA report for EPDs ROCKWOOL Nordics, Feb. 2022
Larisa Xanthopoulou - ROCKWOOL Rules for publishing EPDs, ver.3, December 2021
Program operator and publisher Phone: +47 23 08 80 00
The Norwegian EPD Foundation e-mail: post@epd-norge.no
Post Box 5250 Majorstuen, 0303 Oslo, Norway web: www.epd-norge.no
Owner of the declaration: Phone: +45 4656 1616
ROCKWOOL Nordics e-mail: info@rockwool.com
Hovedgaden 501, DK-2640 Hedehusene web: www.rockwool.dk
Author of the Life Cycle Assessment Phone: +47 916 50 916
LCA.no AS e-mail: post@lca.no
Dokka 6B, 1671 web: www.lca.no
Developer of EPD generator Phone: +47 916 50 916
LCA.no AS e-mail: post@lca.no
Dokka 6B,1671 Kråkerøy web: www.lca.no
ECO Platform web: www.eco-platform.org
ECO Portal web: ECO Portal
11 / 11
