Environmental Product
Declaration
In accordance with ISO 14025 and EN 15804 +A1
NTech outward opening topswing windows 105/80 – TG &
TY (with aluminium cladding)
Owner of the declaration:
NorDan AS Product name:
Program holder and publisher: NTech outward opening
topswing windows 105/80 –
TG & TY (with aluminium
The Norwegian EPD foundation
Declaration number: cladding)
RN eE gP iD s- t3 ra4 t5 i7 o- n2 0 N5 u7 m-E bN
e r: Manufacturer:
NorDan AS
NEPD-3457-2057-EN
Issue date:
Valid to:
02.05.2022
The Norwegian 02.05.2027
EPD Foundation
General information
Product: Owner of the declaration:
NTech outward opening topswing windows 105/80 – TG & TY NorDan AS
(with aluminium cladding) Kontaktperson: Fredrik Jonsson
Tlf: +46 (0) 10-130 01 78
e-post: fredrik.jonsson@nordan.se
Program holder: Manufacturer:
The Norwegian EPD Foundation NorDan sp. z o.o.
Post Box 5250 Majorstuen, 0303 Oslo Fabryczna 16, PL-64-200 Wolsztyn, Poland
Tlf: +47 977 22 020
e-mail: post@epd-norge.no Phone: +48 68 34 70 500
Fax: 048 68 34 73 541
Declaration number: Place of production:
NEPD-3457-2057-EN Wolsztyn, Poland
ECO Platform registration number: Management system:
NorDan sp. z o.o. Works with EN ISO 9001:2015, ISO
14001:2015
This declaration is based on Product Category Rules:
CEN Standard EN 15804 serves as core PCR
NPCR 014:2019 Part B for windows and doors version 3.0 Org. no.:
NO 979 776 233 MVA
Declaration of responsibility: Issue date:
The owner of the declaration shall be responsible for the 02.05.2022
underlying information and evidence. EPD Norway shall not
be responsible with regard to manufacturer information, life
cycle data and evidence.
Valid to:
02.05.2027
Declared unit: Year of study:
2021
Declared unit with option: Comparability:
EPD of construction products may not be comparable if they
are not comply with NS-EN 15804 and seen in a building
context.
Functional unit:
1 window measuring 1.23 m x 1.48 m (reference window based
on EN 14351-1) with an expected service life of 60 yrs. with The EPD has been worked out by:
aluminium cladding. with an essential parameter U-value = Roja Modaresi
0,82W/m2K. Conversion factor is 68.59. [Kg/FU]. Norsk Treteknisk Institutt
Verification:
Independent verification of the declaration and data,
according to ISO14025:2010
internal external
Approved
Third party verifier:
Gaylord K. Booto PhD., Senior Research Scientist, NORSUS AS
(Independent verifier approved by EPD Norway)
NEPD-3457-2057-EN NTech outward opening topswing windows 105/80 – TG & TY (with aluminium cladding)
2/9
Product
Product description: Technical data:
Window with outward opening fully reversible opening sash for use Outward opening window. Triple glazed, 105mm frame with
in exterior walls of domestic and commercial buildings. 8mm aluminium clad, 80mm sash. Uwin 0,82W/m2K.
Certified: BBA, Secured by Design, SP Sitac “P”.
Product specification:
25% of aluminium and 18% of glass is produced from recycled The total weight of the product is 68.59 kg. The packaging
material. has a average weight of 3.2 kg.
Product group TG & TY is covered in this EPD. The highest
amount for constituent material has been used.
Materials kg %
Pine timber 16.57 24.16 Market:
Glass 40.93 59.68 Europe, but scenarios beyond cradle-to-gate are based
Spacer 0.73 1.07 on the situation in the Norwegian market.
Triple glazed Butyl 0.02 0.03
unit Sealant 1.08 1.57
Argon gas 0.07 0.10
Absorbent 0.02 0.03
Paint 0.57 0.83 Reference service life:
Aluminium 1.28 1.86 The reference service life is 60 years for aluminium cladding
Plastic 0.11 0.16 timber frame.
Gasket 0.49 0.71
Metal- Steel alloys 4.26 6.21
Sealant and Glue 0.08 0.12
Aluminium 2.32 3.38
Additional for
Plastic 0.03 0.04
alu clad
Metals 0.03 0.04
Total weight of the product 68.59 100.00
Wood packaging 3.1
Steel packaging 0.05
Plastic packaging 0.08
Total weight with packaging 71.82
LCA: Calculation rules
Functional unit: System boundary:
1 window measuring 1.23 m x 1.48 m (reference window based on All modules are included. Below is a technical flowchart for
EN 14351-1) with an expected service life of 60 yrs. with aluminium the production line at NorDan. Modul D is calculated with
cladding. with an essential parameter U-value = 0,82W/m2K. energy substitution and explained in the scenarios.
Conversion factor is 68.59. [Kg/FU].
NEPD-3457-2057-EN NTech outward opening topswing windows 105/80 – TG & TY (with aluminium cladding)
3/9
Data quality Cut-off criteria:
Data is representative of year 2019 and was collected in 2020- All raw materails and energy use is included. Where data was
2021. Data is taken from processes from Ecoinvent 3.1-3.7. Some available for infrastructure from Ecoinvent, it is included.
processes are based on Ecoinvent v3.1 (2014) and v3.2 (2015), but Example: ‘Metal working factory'. In the production process,
all upstream processes are v3.4 (2017)-3.5 (2018). Remaining data raw materials and energy of low amounts are not included
is based on Ecoinvent v3.7 (2020). "Allocation cut-off by (<1%). These cut-off rules do not apply to dangerous
classification" adjusted to improve representativeness. substances.
Allocation: Calculations of biogenic carbon:
Allocation is done in accordance with the provisions of EN 15804. Sequestration and release of biogenic carbon is included
Allocation of energy, water and waste from production is calculated according to EN 16485:2014. This is based on the modularity
by a physical allocation factor based on the manufacturer input. principle in EN 15804:2012 that specifies that the emissions
For waste produced at the manufacturing, the burdens for reuse, shall be accounted in the module that they occur. The
recycling and recovery is allocated by using this allocation factor. amount of carbon dioxide sequestrated is calulated in
accordance to EN 16449:2014. Timber comes from
sustainable forestry and has FSC certified traceability.
LCA: Scenarios and additional technical information
The following information describe the scenarios in the different modules of the EPD
The transportation from production to construction site is based on a scenario where the product is transported on a large lorry from
Poland to Oslo, Norway (1250 km) and then to a warehouse which is assumed to be in a 250 km radius from Oslo. Transport from
warehouse to a construction site is assumed to be 50 km on a medium truck.
Transport from production place to assembly/user (A4)
Type Capacity utilisation Type of vehicle Distance km Fuel/Energy Fuel/Energy
(incl. return) % consumption pr tkm consumption pr km
Truck 53 EURO5, >32 tonn 1500 0.023 l/tkm 0.31 l/km
Truck 26 EURO5, 16-32 tonn 50 0.045 l/tkm 0.25 l/km
Installation (A5)
Unit Value According to the report from EPD-Norge ‘Harmonising the
Auxiliary kg 0 documentation of scenarios beyond cradle to gate, EN 15804’ there is
Water consumption m3 0 no loss on site during construction activities. The window products in
Electricity consumption MJ 0 this EPD are painted and surface treated in the production and not at
Other energy carriers MJ 0 the building site. Therefore, there is only 2 items left in this module. 1)
Material loss kg 0 Waste treatment of packaging which is considered in the EPD
Output materials from waste treatment kg 3.23 calculations. 1) Energy use during installation. This can be varied
Dust in the air kg 0 depending on the floor, type of building and several other unknown
parameters, and therefore ignored in the calculation.
Maintenance (B2)/Repair (B3)
The maintenance scenario included cleaning, painting and change of
Unit Value (alu cladding) IGU. Cleaning is performed three times per year. It is calculated with
1,5 dl of detergent and 3 litres of water each year. Windows with
Detergents kg 9
aluminium cladding are assumed to be painted 3 times during its
Water consumption l 180
lifetime from inside. It is assumed that 5 gr of lubricating oil is used
Lubricating oil kg 0.30 every year for fittings and moving parts. The glazing unit is changed
Paint kg 0.55 once during the lifetime for the windows with aluminium cladding. No
Transport tkm 2.95 repair is assumed during the product lifetime.
Glazing unit kg 59.43
Synthetic rubber kg 0.49
Transport (IGU) tkm 12.28
NEPD-3457-2057-EN NTech outward opening topswing windows 105/80 – TG & TY (with aluminium cladding)
4/9
Replacement (B4)/Refurbishment (B5)
*Number or RSL (Reference Service Life). The window has RSL of 60
Unit Value years. Therefore, it is assumed to replace the insulated glass unit after
Replacement cycle* yr 60 30 years (See Module B4). There is no need for refurbishment during
Electricity consumption kWh 0 the product lifetime.
Replacement of worn parts 0 0
(C1) As there are no data for de-construction, it is assumed no activites in C1 in this study. The windows are assumed to be treated as
mixed waste and sent to incineration. The combustible materials are then energy recovered, while glass is assumed to end up in the
bottom ash and then landfilled. The metals are usually sorted out of the bottom ash and then recycled, but there is no data of the share
which are recycled and therefore standard values from Ecoinvent is utilized.
The transport of window as waste is calculated based on a scenario with 50 km distance.
Transport to waste processing (C2)
Type Capacity utilisation Type of vehicle Distance km Fuel/Energy Fuel/Energy
(incl. return) % consumption pr tkm consumption pr km
Truck 44 Unspecified 50 0.03l/tkm 0.28 l/km
Windows are assumed to be sorted as mixed construction waste and treated with incineration with energy recovery. However, the
manufacturer has documented the recycling potentials for its product in the Construction Product Declaration eBVD
NorDan TG Vridfönster Trä/Alu 105, ID: C-SE556294452901-67 URL:https://www.ebvd.org/BMI/Document/Export/2952/0/Pdf
NorDan TY Vridfönster Trä/Alu 105, ID: C-SE556294452901-28 URL:https://www.ebvd.org/BMI/Document/Export/1599/0/Pdf In the
documentation, Chapter 10, the specific material recovery, and energy recovery potential is reported for the product.
End of Life (C1, C3, C4)
Unit Value
Hazardous waste disposed kg 0
Collected as mixed construction waste kg 68.59
Reuse kg 0
Recycling kg 3.37
Energy recovery kg 65.22
To landfill kg 0.00
The benefits beyond life cycle has been modelled based on the output flows from module C3. This includes energy from incineration and
scrap metal recovered from the ashes. The amount recovered metal is assumed to avoid production of primary metals in accordance to
6.4.3.3 in EN 15804. The exported energy is substituting Norwegian district heating mix and electricity mix. Inventory processes causing
substitution of avoided virgin raw materials has be constructed for each material.
Benefits and loads beyond the system boundaries (D)
Value (alu
Unit cladding)
Substitution of electricity MJ 186.3
Substitution of thermal energy MJ 1348.7
Substitution of raw materials kg 25.1
NEPD-3457-2057-EN NTech outward opening topswing windows 105/80 – TG & TY (with aluminium cladding)
5/9
LCA: Results
System boundaries (X = included)
Beyond the
system
boundaries
X X X
Environmental impact With alu clad
A4 A5
0.00E+00
6.44E-06
8.49E-02 3.49E-03
ADPM 2.34E-05
EP
ADPM
riapeR
A2
X
Parameter B1 B2
GWP 1.08E+02
ODP
AP
ADPE
Parameter
ODP
AP
-3.28E+03
GWP Global warming potential; ODP Depletion potential of the stratospheric ozone layer; POCP Formation potential of tropospheric
photochemical oxidants; AP Acidification potential of land and water; EP Eutrophication potential; ADPM Abiotic depletion potential for non fossil
resources; ADPE Abiotic depletion potential for fossil resources.
tropsnarT
Global warming potential in A1-A3 includes sequestration of 26.4 kg CO2 as carbon in the wood. This amount is accounted as an
emission in module C3. Additionally, it is included sequestration og 4.5 kg in the wood packaging. This is accounted as an emission
in module A5. The flow of biogenic carbon for the system is presented in page 9.
B4
B3 B5
0.00E+00
noitallatsni
noitcurtsnoC
egats esU
tnemhsibrufeR
End of Life stage
B3 C1 D
X
-yrevoceR-esueR laitnetop
gnilcyceR
Use stage
A1
slairetam
waR
A4
gnissecorp
etsaW
lasopsiD
C4
tnemecalpeR
B7 C2
X X X X X
Unit A1-A3 B4
tropsnarT
esu
ygrene
lanoitarepO
esu
retaw
lanoitarepO
tropsnarT
Construction
Product stage and installation
stage
A3 A5 B1 B2 B6
X X
kg CO -ekv 9.43E+00 4.55E+00 0.00E+00 7.15E+01 0.00E+00
2
1.66E-02 2.00E+00
kg SO -ekv 6.81E-01 2.48E-02 0.00E+00
2
gnirutcafunaM ecnanetniaM
B5
noitcurtsnoc-eD
noitilomed
C3
X X X X X
kg CFC11-ekv 1.84E-06 0.00E+00 0.00E+00 2.40E-06 1.00E+00 0.00E+00 0.00E+00
POCP kg CH -ekv 1.75E-01 1.15E-03 0.00E+00 0.00E+00 0.00E+00 0.00E+00
2 4
0.00E+00 2.33E-01 3.00E+00 0.00E+00 0.00E+00
EP kg PO3--ekv 0.00E+00 0.00E+00 3.43E-02 4.00E+00 0.00E+00 0.00E+00
4
kg Sb-ekv 1.34E-03 0.00E+00 0.00E+00 6.08E-04 5.00E+00 0.00E+00 0.00E+00
MJ 1.69E+03 1.61E+02 0.00E+00 0.00E+00 1.05E+03 6.00E+00 0.00E+00 0.00E+00
Unit B6 B7 C1 C2 C3 C4 D
GWP kg CO -ekv 0.00E+00 0.00E+00 0.00E+00 4.31E-01 3.41E+01 5.40E-01 -3.33E+02
2
kg CFC11-ekv 0.00E+00 0.00E+00 0.00E+00 7.90E-08 4.35E-08 1.44E-07 -1.00E-05
POCP kg CH -ekv 0.00E+00 0.00E+00 0.00E+00 5.44E-05 2.69E-04 1.24E-04 -1.21E-01
2 4
kg SO -ekv 0.00E+00 0.00E+00 0.00E+00 1.36E-03 4.04E-03 3.03E-03 -1.84E+00
2
kg PO3--ekv 0.00E+00 0.00E+00 0.00E+00 2.25E-04 1.25E-03 5.60E-04 -1.65E-01
4
kg Sb-ekv 0.00E+00 0.00E+00 0.00E+00 1.46E-06 1.08E-06 1.08E-06 -8.75E-04
ADPE MJ 0.00E+00 0.00E+00 0.00E+00 6.93E+00 7.92E+01 1.38E+01
NEPD-3457-2057-EN NTech outward opening topswing windows 105/80 – TG & TY (with aluminium cladding)
6/9
Resource use with alu clad
Parameter Unit A1-A3 A4 A5 B1 B2 B3 B4 B5
RPEE MJ 4.9E+02 1.8E+00 0.0E+00 0.0E+00 7.1E+01 0.0E+00 0.0E+00 0.0E+00
RPEM MJ 3.3E+02 0.0E+00 0.0E+00 0.0E+00 0.0E+00 0.0E+00 0.0E+00 0.0E+00
TPE MJ 8.2E+02 1.8E+00 0.0E+00 0.0E+00 7.1E+01 0.0E+00 0.0E+00 0.0E+00
NRPE MJ 1.9E+03 1.6E+02 0.0E+00 0.0E+00 1.1E+03 0.0E+00 0.0E+00 0.0E+00
NRPM MJ 1.0E+02 0.0E+00 0.0E+00 0.0E+00 2.2E+01 0.0E+00 0.0E+00 0.0E+00
TRPE MJ 2.0E+03 1.6E+02 0.0E+00 0.0E+00 1.1E+03 0.0E+00 0.0E+00 0.0E+00
SM kg 1.1E+00 0.0E+00 0.0E+00 0.0E+00 0.0E+00 0.0E+00 0.0E+00 0.0E+00
RSF MJ 9.2E-02 0.0E+00 0.0E+00 0.0E+00 1.0E-01 0.0E+00 0.0E+00 0.0E+00
NRSF MJ 1.4E-01 0.0E+00 0.0E+00 0.0E+00 1.4E-01 0.0E+00 0.0E+00 0.0E+00
W m3 2.2E+00 1.8E-02 0.0E+00 0.0E+00 8.0E-01 0.0E+00 0.0E+00 0.0E+00
Resource use with alu clad
Parameter Unit B6 B7 C1 C2 C3 C4 D
RPEE MJ 0.0E+00 0.0E+00 0.0E+00 8.9E-02 2.8E+02 2.0E-01 -1.2E+03
RPEM MJ 0.0E+00 0.0E+00 0.0E+00 0.0E+00 -2.8E+02 0.0E+00 0.0E+00
TPE MJ 0.0E+00 0.0E+00 0.0E+00 8.9E-02 6.4E-01 2.0E-01 -1.2E+03
NRPE MJ 0.0E+00 0.0E+00 0.0E+00 7.1E+00 8.0E+01 1.4E+01 -3.4E+03
NRPM MJ 0.0E+00 0.0E+00 0.0E+00 0.0E+00 -7.5E+01 0.0E+00 0.0E+00
TRPE MJ 0.0E+00 0.0E+00 0.0E+00 7.1E+00 4.9E+00 1.4E+01 -3.4E+03
SM kg 0.0E+00 0.0E+00 0.0E+00 0.0E+00 0.0E+00 0.0E+00 0.0E+00
RSF MJ 0.0E+00 0.0E+00 0.0E+00 0.0E+00 4.3E-01 0.0E+00 -7.7E+01
NRSF MJ 0.0E+00 0.0E+00 0.0E+00 0.0E+00 2.8E-01 0.0E+00 -4.9E+01
W m3 0.0E+00 0.0E+00 0.0E+00 7.0E-04 1.3E-02 1.2E-02 -5.0E+00
RPEE Renewable primary energy resources used as energy carrier; RPEM Renewable primary energy resources used as raw materials; TPE
Total use of renewable primary energy resources; NRPE Non renewable primary energy resources used as energy carrier; NRPM Non renewable
primary energy resources used as materials; TRPE Total use of non renewable primary energy resources; SM Use of secondary materials; RSF
Use of renewable secondary fuels; NRSF Use of non renewable secondary fuels; W Use of net fresh water.
End of life-Waste with alu clad
Parameter Unit A1-A3 A4 A5 B1 B2 B3 B4 B5
HW kg 3.22E+00 8.32E-03 0.00E+00 0.00E+00 4.72E+01 0.00E+00 0.00E+00 0.00E+00
NHW kg 3.21E+01 1.31E+01 0.00E+00 0.00E+00 1.14E+01 0.00E+00 0.00E+00 0.00E+00
RW kg 2.10E-02 1.05E-03 0.00E+00 0.00E+00 1.83E-02 0.00E+00 0.00E+00 0.00E+00
End of life-Waste with alu clad
Parameter Unit B6 B7 C1 C2 C3 C4 D
HW kg 0.00E+00 0.00E+00 0.00E+00 3.47E-04 5.82E-03 5.16E+01 -2.13E+00
NHW kg 0.00E+00 0.00E+00 0.00E+00 4.28E-01 1.47E-01 4.04E-01 -5.53E+01
RW kg 0.00E+00 0.00E+00 0.00E+00 4.55E-05 1.57E-05 8.23E-05 -4.46E-03
HW Hazardous waste disposed; NHW Non hazardous waste disposed; RW Radioactive waste disposed
End of life- Output flow with alu clad
Parameter Unit A1-A3 A4 A5 B1 B2 B3 B4 B5
CR kg 0.00E+00 0.00E+00 0.00E+00 0.00E+00 0.00E+00 0.00E+00 0.00E+00 0.00E+00
MR kg 8.69E-01 0.00E+00 1.30E-01 0.00E+00 2.34E-01 0.00E+00 0.00E+00 0.00E+00
MER kg 7.10E-02 0.00E+00 3.10E+00 0.00E+00 0.00E+00 0.00E+00 0.00E+00 0.00E+00
EEE MJ 7.51E+00 0.00E+00 0.00E+00 0.00E+00 4.78E+00 0.00E+00 0.00E+00 0.00E+00
ETE MJ 8.30E+01 0.00E+00 0.00E+00 0.00E+00 3.30E+01 0.00E+00 0.00E+00 0.00E+00
End of life- Output flow with alu clad
Parameter Unit B6 B7 C1 C2 C3 C4 D
CR kg 0.00E+00 0.00E+00 0.00E+00 0.00E+00 0.00E+00 0.00E+00 0.00E+00
MR kg 0.00E+00 0.00E+00 0.00E+00 0.00E+00 3.37E+00 0.00E+00 -2.51E+01
MER kg 0.00E+00 0.00E+00 0.00E+00 0.00E+00 0.00E+00 0.00E+00 0.00E+00
EEE MJ 0.00E+00 0.00E+00 0.00E+00 0.00E+00 2.91E+01 0.00E+00 -1.86E+02
ETE MJ 0.00E+00 0.00E+00 0.00E+00 0.00E+00 2.01E+02 0.00E+00 -1.35E+03
CR Components for reuse; MR Materials for recycling; MER Materials for energy recovery; EEE Exported electric energy; ETE Exported thermal
energy
Reading example: 9,0 E-03 = 9,0*10-3 = 0,009
NEPD-3457-2057-EN NTech outward opening topswing windows 105/80 – TG & TY (with aluminium cladding)
7/9
Norwegian additional requirements
Greenhouse gas emissions from the use of electricity in the production phase
National (Poland) market with low-voltage, including production of transmission lines and grid losses, has been used for electricity in
the production process (A3).
Data source Quantity Unit
Ecoinvent v3.7 (september 2020) 1030 gram CO 2-ekv./kWh
Hazardous substances
The product contains no substances from REACH Candidate List or the Norwegian Priority List
The product contains substances below 0.1% by weight on the REACH Candidate List
The product contains substances from REACH Candidate List or the Norwegian Priority List, see table under Specific
Norwegian requirements.
The product does not contain any substances on the REACH Candidate List or the Norwegian Priority List. The product can be
characterized as hazardous waste (according to the Waste Shift, Appendix III), see table under Specific Norwegian
requirements.
Transport
Transport from production site to construction site according to scenario in A4: 1500+50 km
Indoor air quality
The product has not been tested for emissions to indoor environments.
Carbon footprint
To increase the transparency of the climate impacts, the GWP indicator has been divided into sub-indicators:
GWP-IOBC Climate impacts calculated according to instant oxidation principle
GWP-BCIP Climate impacts calculated from the net impacts of sequestration and emission of biogenic carbon
Climate impact with alu clad
Parameter Unit A1-A3 A4 A5 B1 B2 B3 B4 B5
GWP-IOBC kg CO -ekv 1.39E+02 9.43E+00 0.00E+00 0.00E+00 7.15E+01 0.00E+00 0.00E+00 0.00E+00
2
GWP-BCIP kg CO -ekv -3.10E+01 0.00E+00 4.55E+00 0.00E+00 0.00E+00 0.00E+00 0.00E+00 0.00E+00
2
GWP kg CO -ekv 1.08E+02 9.43E+00 4.55E+00 0.00E+00 7.15E+01 0.00E+00 0.00E+00 0.00E+00
2
Climate impact with alu clad
Parameter Unit B6 B7 C1 C2 C3 C4 D
GWP-IOBC kg CO -ekv 0.00E+00 0.00E+00 0.00E+00 4.31E-01 7.69E+00 5.40E-01 -3.33E+02
2
GWP-BCIP kg CO -ekv 0.00E+00 0.00E+00 0.00E+00 0.00E+00 2.64E+01 0.00E+00 0.00E+00
2
GWP kg CO -ekv 0.00E+00 0.00E+00 0.00E+00 4.31E-01 3.41E+01 5.40E-01 -3.33E+02
2
Additional information
For the products with different sizes from the declared unit, the environmental impacts must be converted by using a conversion
factor. The Norwegian EPD Foundation has published instructions on how to interpret EPDs for windows on its website (www.epd-
norge.no) where different calculation methods have been stated. (Document: Bruksanvisninger i hvordan tolke EPD'er – Vinduer)
NEPD-3457-2057-EN NTech outward opening topswing windows 105/80 – TG & TY (with aluminium cladding)
8/9
Bibliografi
NS-EN ISO 14025:2010 Miljømerker og deklarasjoner - Miljødeklarasjoner type III - Prinsipper og prosedyrer.
NS-EN ISO 14044:2006 Miljøstyring - Livsløpsvurderinger - Krav og retningslinjer
NS-EN 15804:2012+A1:2013 Bærekraftig byggverk - Miljødeklarasjoner - Grunnleggende produktkategoriregler for
byggevarer
ISO 21930:2007 Sustainability in building construction - Environmental declaration of building products
Modaresi, R. 2020 LCA-report for Nordan LCA-report nr. 325039-1 from Norwegian Institute of Wood
Technology, Oslo, Norway.
NPCR014 (04/2019) Product category rules for windows and doors, rev3, April 2019
NS-EN 16485:2014 Tømmer og skurlast - Miljødeklarasjoner - Produktkategoriregler for tre og trebaserte produkter
til bruk i byggverk
NS-EN 16449:2014 Tre og trebaserte produkter - Beregning av biogent karboninnhold i tre og omdanning til
karbondioksid
Ecoinvent v3.0-3.7 Ecoinvent database version 3.0-3.7 Centre for Life Cycle Inventories.
Statistisk sentralbyrå Tabell 04727: Fjernvarmebalansen, 2015
Statistisk sentralbyrå Tabell 09469: Nettoproduksjon av fjernvarme, 2015
NEPD-307-179-NO EPD for skurlast av gran eller furu. Treindustrien
Bruksanvisninger i hvordan tolke EPD'er – Vinduer. https://www.epd-norge.no [in Norwegian]
Program operator and publisher Tlf: +47 23 08 80 00
The Norwegian EPD Foundation
Postboks 5250 Majorstuen, 0303 Oslo e-post: post@epd-norge.no
Norway web www.epd-norge.no
Owner of the declaration Tlf: +47 51 40 40 00
NorDan AS
Stasjonsveien 46, N-4460 Moi e-post: firmapost@nordan.no
Norway
web www.nordan.no
Author of the Life Cycle Assessment Tlf: +47 98 85 33 33
Roja Modaresi
Norsk Treteknisk Instiutt e-post: firmapost@treteknisk.no
Postboks 113 Blindern, 0314 Oslo, Norway web www.treteknisk.no
NEPD-3457-2057-EN NTech outward opening topswing windows 105/80 – TG & TY (with aluminium cladding)
9/9
EPD for the best
environmental
decision
www.epd-norge.no
The Norwegian EPD foundation
EPD for the best environmental decision
12
