ENVIRONMENTAL PRODUCT DECLARATION
-in accordance with ISO 14025, ISO 21930:2017 and EN 15804:2012+2013:A1
Owner of the declaration: Saint-Gobain Denmark A/S ISOVER
Program operator: The Norwegian EPD Foundation
Publisher: The Norwegian EPD Foundation
Declaration number: NEPD-2014-891-EN
Registration number: NEPD-2014-891-EN
ECO Platform reference number: -
Issue date: 13.02.2020
Valid to: 13.02.2025
ISOVER CLIMCOVER Lamella Alu2
Saint-Gobain Denmark A/S, ISOVER
www.epd-norge.no
NEPD-2014-891-EN ISOVER CLIMCOVER Lamella Alu2
General information
Product
Owner of the declaration
ISOVER CLIMCOVER Lamella Alu2
Saint-Gobain Denmark A/S, ISOVER
Program operator
Contact person: Helene Løvkvist Andersen
The Norwegian EPD Foundation
Phone: +45 26 79 57 01
Post Box 5250 Majorstuen, 0303 Oslo
E-mail: Helene.lovkvist.andersen@saint-
Phone: +47 97722020
gobain.com
E-mail: post@epd-norge.no
Web: www.epd-norge.no
Manufacture
Declaration number Saint-Gobain Denmark A/S, ISOVER
NEPD-2014-891-EN
Place of production
ECO Platform reference number Vamdrup, Denmark
Place of usage
Denmark
This declaration is based on Product Category
Rules
Management system
CEN Standard EN 15804:2012 + 2013:A1 serve as
core PCR. The Product Category Rules, NPCR DS/EN ISO 9001
DS/EN ISO 14001
Construction products and services – Part A – (2017)
DS/EN ISO 50001
and NPCR 012 Thermal insulation products – Part B
DS/ISO 45001
(2018) are used in addition to the core PCR.
Org. No.
Statement of liability
1020917543
The owner of the declaration shall be liable for the
underlying information and evidence.
Issue date
EPD Norway shall not be liable with respect to
13.02.2020
manufacturer information, life cycle assessment data
and evidences.
Valid to
13.02.2025
Declared unit
1 m² with a thermal resistance of 1,0 m²K/W with a
Year of study
thickness of 37 mm.
2019
Functional unit
Comparability
1 m² with a thermal resistance of 1,0 m²K/W with a
EPD of construction products may not be
reference service life of 60 years.
comparable, if they do not comply with
EN15804:2012 +2013:A1 and seen in a building
Verification
context.
Independent verification of calculation data and other
environmental information and test of the computer
program was carried out by Martin Erlandsson in
The EPD has been worked out by
accordance with ISO14025, 8.1.3 and 8.1.4 + EN
The EPD has been worked out by the use of the
15804:2012+2013:A1
EPD tool GaBi, version 8.7 by Saint-Gobain LCA
central team and by Helene Løvkvist Andersen,
Externally
Saint-Gobain Denmark A/S.
Company-specific data has been verified by
Saint-Gobain central LCA team and by Hans
Ramsing Orehøj, Saint-Gobain Denmark A/S,
ISOVER
Approved
IVL Swedish Environmental Research Institute
(Independent verifier approved by EPD Norway)
2
NEPD-2014-891-EN ISOVER CLIMCOVER Lamella Alu2
Product description
Product description and description of use:
This EPD describes the potential environmental impacts of 1 m² of glass wool insulation, ISOVER
CLIMCOVER Lamella Alu2, with a thermal resistance equal to 1,00 m2K/W
The intended use of this EPD is to communicate scientifically based environmental information for
construction products, for the purpose of assessing the environmental performance of buildings.
ISOVER glass wool products are CE-labelled according to EN 13162 (2012) “Thermal Insulation
Products for Buildings. Factory made mineral wool (MW) Products. Specification”, and EN 13172
(2011) “Thermal Insulation Products – Evaluation of Conformity”
The production site of Saint-Gobain Denmark A/S, ISOVER in Vamdrup, Denmark, uses a small
amount of natural and abundant raw materials (sand, soda, limestone, feldspar) and a high share of
recycled glass cullets (more than 50 % of external glass cullets). This material is converted by using
fusion and fiberizing techniques to produce glass wool. The products obtained come in the form of
"mineral wool slabs, rolls or lamellas" consisting of a soft, airy structure.
On Earth, naturally, the best insulator is dry immobile air at 10 °C: its thermal conductivity factor,
expressed in λ, is 0,025 W/(mK) (watts per meter Kelvin degree). The thermal conductivity of mineral
wool is close to immobile air as its lambda varies from 0,030 W/(mK) for the most efficient, to 0,040 W/
(mK) to the least efficient.
With its entangled structure, glass wool is a porous material that traps the air, making it one of the best
insulating materials. The porous and elastic structure of the wool also absorbs airborne noise, impact
noise and offers acoustic correction inside premises.
Glass wool containing incombustible materials does not react to fire.
Glass wool insulation is used in buildings as well as industrial facilities. It ensures a high level of
comfort and minimizes carbon dioxide (CO ) emissions by preventing heat loss through roofs, walls,
2
floors, pipes and boilers. It reduces noise and protects homes and industrial facilities against fire.
Correctly installed glass wool products and solutions do not require maintenance, and last throughout
the lifetime of the building (which is set at 60 years as a default value in the model), or as long as the
insulated building component is a part of the building.
2
NEPD-2014-891-EN ISOVER CLIMCOVER Lamella Alu2
Technical data/physical characteristics:
The thermal resistance of the product: 1,00 m2K/W
The thermal conductivity of the product: 0,037 W/(mK)
Reaction to fire: Euroclass A2-s1, d0
Description of the main product components and/or materials:
Mineral wool 92-100 % (REACH registration number 01-2119472313-44-0039)
Binder ≤ 8 %
Description of the main components and/or materials for 1 m2 of product with a thermal
resistance of 1 m2K/W for the calculation of the EPD:
PARAMETER VALUE
Quantity of mineral wool 1 kg
Thickness of mineral wool 37 mm
Surfacing Aluminium polyethylene: 85 g/m²
Polyethylene with and without print: 25 g/m²
Stretch film: 5 g/m²
Packaging for the transportation and distribution
Wood pallet: 189 g/m²
Product used for the Installation None
LCA calculation information
FUNTIONAL UNIT Providing a thermal insulation on 1 m² with a thermal
resistance of equals 1 m2K/W
SYSTEM BOUNDARIES
Cradle to Grave
REFERENCE SERVICE LIFE (RSL) 60 years
(with correct installation, the product has same RSL as the building component)
CUT-OFF RULES See detailed explanation page 10
ALLOCATIONS
See detailed explanation page 10
Renewable electricity mix (reference year 2018)
ELECTRICITY USED FOR THE
GO’s from LOS, contracted 2018 – 2020, to be prolonged to be valid at
MANUFACTORING PROCESS least equal to the validity of this EPD.
GEOGRAPHICAL COVERAGE AND TIME
PERIOD Denmark, 2018
GREENHOUSE GAS EMISSION
FROM ELECTRICITY
Which equals 0,035 kg CO2 equiv /kWh
3
NEPD-2014-891-EN ISOVER CLIMCOVER Lamella Alu2
Flow diagram of the Life Cycle
A1-A3 Product stage A4-A5 Construction process
Sand and other Facing: variable A1-A3 Production
minerals according to product Diesel Additional
production due to
losses 2%
Cullet Wood pallet and
Polyethylene
Binder packaging
A1 – A3 Production A4 A5
Transport Installation
Internal
Natural Gas recycling
Electricity Primary product
Diesel
Evaporation
Water
Air
Waste Emission
Losses: 2%
Packaging waste
External
Landfill Recycling
B1-B7 Use C1-C4 End-of-life
Diesel
B1-B5 use B6-B7 operation C1 de- C2 transport C3 waste C4 disposal
of the building construction, to waste processing
demolition processing for reuse,
recovery
and/or
recycling
Waste (glass
wool product):
100%
Landfilled
4
NEPD-2014-891-EN ISOVER CLIMCOVER Lamella Alu2
System boundaries (X = included, MND = Module not declared)
Beyond the
Construction
Product stage Use stage End of life stage system
installation stage
boundaries
5
slairetam
waR
tropsnarT
gnirutcafunaM
tropsnarT
noitallatsni
noitcurtsnoC
egats esU
ecnanetniaM
riapeR
tnemecalpeR tnemhsibrufeR
esu
ygrene
lanoitarepO
esu
retaw
lanoitarepO
noitcurtsnoc-eD
noitilomed tropsnarT
gnissecorp
etsaW
lasopsiD
-yrevoceR-esueR laitnetop-gnilcyceR
A1 A2 A3 A4 A5 B1 B2 B3 B4 B5 B6 B7 C1 C2 C3 C4 D
X X X X X X X X X X X X X X X X MND
Product stage, A1- A3
Description of the stage:
The product stage of the mineral wool products is subdivided into 3 modules A1, A2 and A3
respectively “Raw material supply”, “transport” and “manufacturing”.
The aggregation of the modules A1, A2 and A3 is a possibility considered by the EN
15804:2012+2013:A1 standard. This rule is applied in this EPD.
A1, Raw material supply
This module takes into account the extraction and processing of all raw materials and energy which
occur upstream to the studied manufacturing process.
Specifically, the raw material supply covers production of binder components and sourcing (quarry) of
raw materials for fiber production, e.g. sand and borax for glass wool. Besides these raw materials,
glass cullet is also used as input.
About cullet: The main raw material for the production of glass insulation material is cullets or/and
sand. Only specific cleaning activities and transport is included for the cullets – and thus not the
impacts from the full life cycle of glass. The reason is that cullets are considered a waste product and
not initially produced for the purpose of glass wool insulation production.
The only activities included are:
- Magnetic separation of metallic piece
- Separation of other piece-crushing of glass (<20 mm)
- Separation of bottle cap crushing (<2 mm) sieving
- Transport
A2, Transport to the manufacturer
The raw materials are transported to the manufacturing site. In our case, the modeling includes: road
and boat transportations (specific values) of each raw material.
A3, Manufacturing
This module covers glass wool fabrication, including melting and fiberizing (see process flow diagram).
In addition, the production of packaging material is taking into account at this stage.
NEPD-2014-891-EN ISOVER CLIMCOVER Lamella Alu2
Manufacturing process flow diagram
Construction process stage, A4- A5
Description of the stage:
The construction process is divided into 2 modules: A4, transport to the building site and A5,
installation in the building.
Description of scenarios and additional technical information:
A4, Transport to the building site:
This module includes transport from the production gate to the building site.
Transport is calculated on the basis of a scenario with the parameters described in the following table.
PARAMETER VALUE
Fuel type and consumption of vehicle or vehicle
Average truck trailer with a 24t payload, diesel
type used for transport e.g. long distance truck,
consumption 38 liters for 100 km
boat, etc.
Distance 125 km
10 % of the capacity in weight
Capacity utilisation (including empty returns)
30 % of empty returns capacity in weight
Bulk density of transported products 28 kg/m3 (uncompressed density)
Weight capacity utilisation factor 0,415 (by default)
6
NEPD-2014-891-EN ISOVER CLIMCOVER Lamella Alu2
A5, Installation into the building:
This module includes:
- Wastage of products: 2 %. These losses are landfilled (landfill model for glass, see
chapter End-of-life)
- Additional production processes to compensate for the loss
- Processing of packaging wastes: they are 100 % collected and modeled as recovered
matter.
This module does not include:
- Energy for installation of the insulation, as the installation is done manually, and do not
require energy.
PARAMETER VALUE
Wastage of materials on the building site before
waste processing, generated by the product’s 2 %
installation (specified by type)
Output materials (specified by type) as results of Packaging wastes are 100 % collected and modeled
waste processing at the building site e.g. of as recovered matter
collection for recycling, for energy recovering,
disposal (specified by route) Glass wool losses are landfilled
Use stage (excluding potential savings), B1- B7
Description of the stage:
The use stage is divided into the following modules:
- B1: Use
- B2: Maintenance
- B3: Repair
- B4: Replacement
- B5: Refurbishment
- B6: Operational energy use
- B7: Operational water use
Description of scenarios and additional technical information:
Once installation is complete, no actions or technical operations are required during the use stages
until the end-of-life stage. Therefore, glass wool insulation products have no impact (excluding
potential energy savings) on this stage.
7
NEPD-2014-891-EN ISOVER CLIMCOVER Lamella Alu2
End-of-life stage, C1- C4
Description of the stage:
The stage includes the following different modules of end-of-life:
C1, De-construction, demolition
The de-construction and/or dismantling of insulation products are part of the demolition of the entire
building, and are assumed to be made manually. In our case, the environmental impact is assumed to
be very small and can be neglected.
C2, Transport to waste processing
Transport is included and calculated on the basis of a scenario with the parameters described in the
End-of-life table below.
C3, Waste processing for reuse, recovery and/or recycling
Today the product is considered to be landfilled without reuse, recovery or recycling.
C4, Disposal
The glass wool is assumed to be 100% landfilled.
Description of scenarios and additional technical information: See below
PARAMETER DESCRIPTION
The entire insulation product (wool and surfacing) is
Collection process specified by type
collected with mixed construction waste
Recovery system specified by type No re-use, recycling or energy recovery
The entire insulation product (wool and surfacing) is
Disposal specified by type
landfilled
Average truck trailer with a 24t payload, diesel
Assumptions for scenario development (e.g. consumption 38 liters for 100 km.
transportation) 25 km (default distance from the building site to
landfill).
Reuse/recovery/recycling potential, D
Description of the stage: For module D we only take into consideration the materials used within the
product, and not e.g. packaging.
8
NEPD-2014-891-EN ISOVER CLIMCOVER Lamella Alu2
LCA results
LCA model, aggregation of data and potential environmental impact are calculated from the GaBi
software 8.7 and CML impact method has been used, together with Thinkstep 8.7 (2018) and
ecoinvent V3.1 (2014) databases to obtain the inventory of generic data.
Following the “Default international characterization method” specified in ISO21930:2017, biogenic
carbon is not reported in the context of GWP-GHG.
Raw materials and energy consumption, as well as transport distances, have been taken directly from
the manufacturing plant of Saint-Gobain Denmark A/S, ISOVER in Vamdrup (Production data
according 2018).
Resume of the LCA results detailed on the following tables.
Cut-off criteria
The cut-off criterion used in Saint-Gobain EPD will be the mass criterion with the following details:
- Taking into account all input and output flows in a unit process i.e. taking into account the
value of all flows in the unit process and the corresponding LCI whenever available
- No simplification of the LCI by additional exclusions of material flows
Data collected at the manufacturing site was used. The inventory process in this LCA includes all data
related to raw material, packaging material and consumable items, and the associated transport to the
manufacturing site. Process energy and water use, direct production waste and emissions to air and
water are included. Scenarios have been developed to account for downstream processes such as
demolition and waste treatment in accordance with the requirements of EN 15804:2012+A1:2013
All inputs and outputs to the manufacturing plants have been included and made transparent. All
assumptions regarding the materials and water balances have also been included.
All hazardous and toxic materials and substances are considered in the inventory even though they
are below the cut off criteria.
There are excluded processes in the inventory:
- Flows related to human activities, such as employee transport and administration activity, are
according to the PCR not accounted for.
Allocation
Allocation criteria are based on mass.
The allocation of all the air emissions, wastes and energy usage are based on mass (kg). The reason
we can use a mass basis is because we use the exact same manufacturing process shown for every
product. We only produce glass mineral wool at the Vamdrup site using the same process and
therefore all the factors can be allocated by a mass basis.
The amount of binder varies for different products, and is accounted for.
A mass balance was conducted for the 2018 production year to ensure that we haven’t excluded any
materials, emissions and hence potential environmental impacts. Regarding the mass balance, all the
raw materials and corresponding production goods and wastes generated were taken into account.
9
NEPD-2014-891-EN ISOVER CLIMCOVER Lamella Alu2
Influence of particular thicknesses
The results in the tables of this EPD refer to ISOVER CLIMCOVER Lamella Alu2 with a thickness of
37 mm for a functional unit of 1 m² with a thermal resistance equals to 1,00 m2K/W
This EPD includes a range of thicknesses between 20 mm and 120 mm.
For every thickness, use a multiplication factor in order to obtain the environmental performance of
every thickness. Using the thickness factor will for some indicators give higher values than calculated
for the specific thickness in GaBi.
In order to calculate the multiplication factors, a reference unit has been selected (value of R= 1,00
m2K/W for 37 mm). Multiplication factors are obtained by making the LCA calculations for all
thicknesses, including packaging.
In order to obtain the environmental performance associated with the specific product and thickness,
the results expressed in this EPD must be multiplied by its corresponding multiplication factor.
PRODUCT THICKNESS THERMAL
MULTIPLICATION FACTOR
(mm) RESISTANCE
20 0,54 0,72
30 0,81 0,88
37 1,00 1,00
40 1,08 1,06
50 1,35 1,25
60 1,62 1,46
70 1,89 1,66
80 2,16 1,86
90 2,43 2,10
100 2,7 2,24
120 3,24 2,56
Influence of transportation to others countries
The results of stage A4 (transportation of product) in the table of this EPD refer to transportation in
Denmark. This product might also be delivered to the countries in the table below. In order to adapt
the impact of transportation in the A4 column, figures from the current EPD shall be multiply by the
multiplication factors below.
COUNTRY AVERAGE DISTANCE MULTIPLICATION FACTOR
Denmark 125 km (truck) 1,00
Norway 777 km (truck) 100 km (boat) 6,35
Sweden 761 km (truck), 10 km (boat) 6,11
Finland 389 (truck), 1225 km (boat) 4,57
Transport include transportation to ISOVER plant, and average distance from plant to building site.
10
NEPD-2014-891-EN ISOVER CLIMCOVER Lamella Alu2
ENVIRONMENTAL IMPACTS
Product Construction
Use stage End-of-life stage
stage process stage
Parameters
11
3A
/
2A
/
1A
tropsnarT
4A
noitallatsnI
5A
esU
1B
ecnanetniaM
2B
riapeR
3B
4B
tnemecalpeR
5B
tnemhsibrufeR lanoitarepO
6B
esu
ygrene
lanoitarepO
7B
esu
retaw 1C
/ noitcurtsnoceD noitilomed tropsnarT
2C
etsaW
3C
gnissecorp lasopsiD
4C
,yrevocer
,esueR
D
gnilcycer
1,40E+00 1,53E-02 1,55E-03 0 0 0 0 0 0 0 0,00E+00 6,65E-03 0 1,81E-02 0
Global Warming Potential
(GWP) - kg CO equiv/FU
2 The global warming potential of a gas refers to the total contribution to global warming resulting from the emission
of one unit of that gas relative to one unit of the reference gas, carbon dioxide, which is assigned a value of 1.
7,96E-08 2,34E-18 1,59E-11 0 0 0 0 0 0 0 0,00E+00 5,77E-15 0 1,01E-16 0
Ozone Depletion (ODP)
kg CFC-11 equiv/FU Destruction of the stratospheric ozone layer which shields the earth from ultraviolet radiation harmful to life.
This destruction of ozone is caused by the breakdown of certain chlorine and/or bromine containing compounds (chlorofluorocarbons or halons),
which break down when they reach the stratosphere and then catalytically destroy ozone molecules.
1,00E-02 6,52E-05 7,33E-06 0 0 0 0 0 0 0 0,00E+00 2,79E-05 0 1,03E-04 0
Acidification potential (AP)
kg SO equiv/FU
2 Acid depositions have negative impacts on natural ecosystems and the man-made environment incl. buildings.
The main sources for emissions of acidifying substances are agriculture and fossil fuel combustion used for electricity production, heating and transport.
Eutrophication potential (EP) 4,05E-03 1,60E-05 2,10E-06 0 0 0 0 0 0 0 0,00E+00 6,75E-06 0 1,17E-05 0
kg (PO)3- equiv/FU
4
Excessive enrichment of waters and continental surfaces with nutrients, and the associated adverse biological effects.
Photochemical ozone 6,65E-04 2,39E-06 3,32E-07 0 0 0 0 0 0 0 0,00E+00 1,03E-06 0 8,48E-06 0
creation (POPC)
kg Ethene equiv/FU Chemical reactions brought about by the light energy of the sun.
The reaction of nitrogen oxides with hydrocarbons in the presence of sunlight to form ozone is an example of a photochemical reaction.
Abiotic depletion potential for
non-fossil resources (ADP- 1,15E-04 2,03E-10 2,31E-08 0 0 0 0 0 0 0 0,00E+00 8,99E-11 0 6,12E-09 0
elements) - kg Sb equiv/FU
Abiotic depletion potential for
2,13E+01 2,13E-01 2,20E-02 0 0 0 0 0 0 0 0,00E+00 9,26E-02 0 2,40E-01 0
fossil resources (ADP-fossil
fuels) - MJ/FU
Consumption of non-renewable resources, thereby lowering their availability for future generations.
NEPD-2014-891-EN ISOVER CLIMCOVER Lamella Alu2
RESOURCE USE
Product Construction
Use stage End-of-life stage
stage process stage
Parameters
12
3A
/
2A
/
1A
tropsnarT
4A
noitallatsnI
5A
esU
1B
ecnanetniaM
2B
riapeR
3B
4B
tnemecalpeR
5B
tnemhsibrufeR lanoitarepO
6B
esu
ygrene
lanoitarepO
7B
esu
retaw 1C
/ noitcurtsnoceD noitilomed tropsnarT
2C
etsaW
3C
gnissecorp lasopsiD
4C
,yrevocer
,esueR
D
gnilcycer
Use of renewable primary
energy excluding renewable
1,89E+01 4,9E-03 4,2E-03 0 0 0 0 0 0 0 0 2,4E-03 0 3,2E-02 0
primary energy resources used
as raw materials - MJ/FU
Use of renewable primary
energy used as raw materials 3,22E+00 0 6,4E-04 0 0 0 0 0 0 0 0 0 0 0 0
MJ/FU
Total use of renewable primary
energy resources (primary energy
2,21E+01 4,9E-03 4,9E-03 0 0 0 0 0 0 0 0 2,4E-03 0 3,2E-02 0
and primary energy resources used
as raw materials) - MJ/FU
Use of non-renewable primary
energy excluding non-renewable
2,37E+01 2,1E-01 2,3E-02 0 0 0 0 0 0 0 0 9,3E-02 0 2,5E-01 0
primary energy resources used
as raw materials - MJ/FU
Use of non-renewable primary
energy used as raw materials - 2,89E+00 0 5,8E-04 0 0 0 0 0 0 0 0 0 0 0 0
MJ/FU
Total use of non-renewable primary
energy resources (primary energy
2,66E+01 2,1E-01 2,3E-02 0 0 0 0 0 0 0 0 9,3E-02 0 2,5E-01 0
and primary energy resources used
as raw materials) - MJ/FU
Use of secondary material
kg/FU
6,70E-01 0 1,3E-04 0 0 0 0 0 0 0 0 0 0 0 0
Use of renewable secondary
0 0 0 0 0 0 0 0 0 0 0 0 0 0 0
fuels - MJ/FU
Use of non-renewable
0 0 0 0 0 0 0 0 0 0 0 0 0 0 0
secondary fuels - MJ/FU
Use of net fresh water - m3/FU 1,75E-02 1,6E-06 3,7E-06 0 0 0 0 0 0 0 0 7,7E-07 0 6,2E-05 0
NEPD-2014-891-EN ISOVER CLIMCOVER Lamella Alu2
WASTE CATEGORIES
Product Construction
Use stage End-of-life stage
stage process stage
Parameters
13
3A
/
2A
/
1A
tropsnarT
4A
noitallatsnI
5A
esU
1B
ecnanetniaM
2B
riapeR
3B
4B
tnemecalpeR
5B
tnemhsibrufeR lanoitarepO
6B
esu
ygrene
lanoitarepO
7B
esu
retaw 1C
/ noitcurtsnoceD noitilomed tropsnarT
2C
etsaW
3C
gnissecorp lasopsiD
4C
,yrevocer
,esueR
D
gnilcycer
Hazardous waste disposed
3,34E-08 7,66E-10 7,11E-11 0 0 0 0 0 0 0 0,00E+00 3,33E-10 0 4,23E-09 0
kg/FU
Non-hazardous waste disposed
1,00E-01 2,59E-06 2,95E-04 0 0 0 0 0 0 0 0,00E+00 1,23E-06 0 1,15E+00 0
kg/FU
Radioactive waste disposed
4,59E-04 2,49E-07 1,13E-07 0 0 0 0 0 0 0 0,00E+00 1,08E-07 0 3,29E-06 0
kg/FU
NEPD-2014-891-EN ISOVER CLIMCOVER Lamella Alu2
OUTPUT FLOWS
Product Construction
Use stage End-of-life stage
stage process stage
Parameters
14
3A
/
2A
/
1A
tropsnarT
4A
noitallatsnI
5A
esU
1B
ecnanetniaM
2B
riapeR
3B
4B
tnemecalpeR
5B
tnemhsibrufeR lanoitarepO
6B
esu
ygrene
lanoitarepO
7B
esu
retaw 1C
/ noitcurtsnoceD noitilomed tropsnarT
2C
etsaW
3C
gnissecorp lasopsiD
4C
,yrevocer
,esueR
D
gnilcycer
Components for re-use
0 0 0 0 0 0 0 0 0 0 0 0 0 0 0
kg/FU
Materials for recycling
kg/FU
2,30E-02 0 2,19E-01 0 0 0 0 0 0 0 0 0 0 0 0
Materials for energy recovery
0 0 0 0 0 0 0 0 0 0 0 0 0 0 0
kg/FU
Exported energy
0 0 0 0 0 0 0 0 0 0 0 0 0 0 0
MJ/FU
NEPD-2014-891-EN ISOVER CLIMCOVER Lamella Alu2
Product Transport Installation Use End-of-life
(A1-A3) (A4) (A5) (B) (C) Total Recycling
Environmental Positive benefits
impacts of the of recycling
product (D)
Global warming 1,50 1,40
1,00 1,44
0,50
0,02 0,00 0,00 0,02 0,00
0,00
Non-renewable resources 30,00
consumption [1] 21,30
20,00 21,87
10,00
0,21 0,02 0,00 0,33 0,00
0,00
Energy consumption [2] 60,00 48,70
40,00 49,32
20,00
0,22 0,03 0,00 0,37 0,00
0,00
Water consumption [3] 0,02 0,0175
0,02
0,018
0,01
0,01
0,0000 0,0000 0,0000 0,0001 0,00
0,00
Waste production [4] 1,50
1,15
1,00 1,25
0,50
0,10
0,00 0,00 0,00 0,00
0,00
[1] This indicator corresponds to the abiotic depletion potential of fossil resources.
[2] This indicator corresponds to the total use of primary energy.
[3] This indicator corresponds to the use of net fresh water.
[4] This indicator corresponds to the sum of hazardous, non-hazardous and radioactive waste disposed.
Global Warming Potential (Climate Change) (GWP)
When analyzing the above figure for GWP, it can clearly be seen that the majority of contribution to this environmental impact
is from the production modules (A1 – A3). This is primarily because the sources of greenhouse gas emissions are predominant
in this part of the life cycle. CO is generated upstream from the production of electricity and is also released on site by the
2
combustion of natural gas. We can see that other sections of the life cycle also contribute to the GWP; however, the production
modules contribute to over 80% of the contribution. Combustion of fuel in transport vehicles will generate the second highest
percentage of greenhouse gas emissions together the waste during the installation stage.
Non-renewable resources consumptions
We can see that the consumption of non-renewable resources is once more found to have the highest value in the production
modules. This is because a large quantity of natural gas is consumed within the factory, and non-renewable fuels such as
natural gas and coal are used to generate the large amount of electricity we use. The contribution to this impact from the
other modules is very small and primarily due to the non – renewable resources consumed during transportation.
Energy Consumptions
As we can see, modules A1 – A3 have the highest contribution to total energy consumption. Energy in the form of electricity
and natural gas is consumed in a vast quantity during the manufacture of glass mineral wool so we would expect the
production modules to contribute the most to this impact category.
Water Consumption
As we don’t use water in any of the other modules (A4 – A5, B1 – B7, C1 – C4), we can see that there is no contribution to
water consumption. For the production phase, water is used within the manufacturing facility and therefore we see the highest
contribution here. However, we recycle a lot of the water on site so the contribution is still relatively low.
Waste Production
Waste production does not follow the same trend as the above environmental impacts. The largest contributor is the end of
life module. This is because the entire product is sent to landfill once it reaches the end of life state. However, there is still an
impact associated with the production module since we do generate waste on site. The following small impact associated with
installation is due to the loss rate of product during implementation.
15
UF/viuqe2OC
gk
UF/JM
UF/JM
UF/3m
UF/gk
LCA interpretation
kg COequiv/FU 2
MJ/FU
MJ/FU
m3/FU
kg/FU
NEPD-2014-891-EN ISOVER CLIMCOVER Lamella Alu2
Additional information
Additional Norwegian requirements
Greenhouse gas emissions from the use of electricity in the manufacturing phase
The LCA calculation has been made taking into account the fact that during the manufacturing process it is used
100% renewable electricity. This 100% renewable electricity bought is evidenced by Guarantee of Origin certificates
(GOs) from LOS, valid from 2018 to 2020. Will be prolonged to be valid at least equal to the validity of this EPD.
TYPE OF INFORMATION DESCRIPTION
Location Representative of average production in Denmark
Geographical Split of energy sources in Denmark
representativeness -Hydro: 54%
description -Biomass: 46%
Reference year 2018
Type of data set Cradle to gate from Thinkstep database
Gabi database from International Energy Agency -2013
Source
Guarantee of Origin certificates (GOs) – valid from 2018
Electricity mix (from renewable sources)
Denmark
46%
54%
Biomass Hydro
The dataset used to model the renewable electricity mix used for these calculations come from thinkstep and
ecoinvent database.
DATA SOURCE AMOUNT UNIT
thinkstep (2018) and
0,035 kg CO2 equiv /KWh
ecoinvent 3.1 (2014)
Indoor environment
The EPD does not give any information on release of regulated dangerous substances to indoor air, because the
national regulation in Denmark does not require any verification and declaration of release of regulated
dangerous substances today.
Dangerous substances
The product contains no substances given from the REACH Candidate list (of 15.01.2018)
(REACH registration number 01-2119472313-44-0039)
16
NEPD-2014-891-EN ISOVER CLIMCOVER Lamella Alu2
Bibliography
- Product-Category Rules:
o NPCR Construction products and services – Part A (2017)
o NPCR 012 Thermal insulation products – Part B (2018)
- Environmental labels and declarations - Type III environmental declarations -Principles and
procedures (ISO 14025:2006)
- Environmental management - Life cycle assessment – Requirements and guidelines (ISO
14044:2006)
- Sustainability of construction works - Environmental product declaration - Core rules for the
product category of construction products (EN 15804:2012+2013:A1)
- Sustainability in building construction - Environmental declaration of building products (ISO
21930:2017)
- LCA report Saint-Gobain ISOVER 2019, author: Saint-Gobain + Saint-Gobain Denmark A/S
- Ecoinvent database V3.1 (2014)
- GaBi 8.7 - database (2018)
- Guarantee of Origin certificates (GOs) from LOS, issued to Saint-Gobain (2018)
Program operator and publisher Phone: +47 97722020
The Norwegian EPD Foundation E-mail: post@epd-norge.no
Post Box 5250 Majorstuen, 0303 Oslo
Norway
Web: www.epd-norge.no
Owner of the declaration Phone: +45 26 79 57 01
Saint-Gobain Denmark A/S ISOVER E-mail: Helene.Lovkvist.Andersen@saint-
Østermarksvej 4, 6580 Vamdrup gobain.com
Denmark Web: www.isover.dk
Phone: +33 645 614 089
Author of the Life Cycle Assessment
E-mail: Yves.Coquelet@saint-gobain.com
Saint-Gobain, Central Marketing &
Development
Web: www.saint-gobain.com
17
NEPD-2014-891-EN ISOVER CLIMCOVER Lamella Alu2
