Environmental product declaration
in accordance with ISO 14025 and EN 15804+A2
Isola Takshingel Premium Rett
OOwwnneerr ooff tthhee ddeeccllaarraattiioonn:: PPrrooggrraamm ooppeerraattoorr::
Isola AS The Norwegian EPD Foundation
PPrroodduukktt:: DDeeccllaarraattiioonn nnuummbbeerr::
Isola Takshingel Premium Rett
NEPD-8335-8004-EN
DDeeccllaarreedd uunniitt::
1 m2 RReeggiissttrraattiioonn nnuummbbeerr::
TThhiiss ddeeccllaarraattiioonn iiss bbaasseedd oonn PPrroodduucctt CCaatteeggoorryy NEPD-8335-8004-EN
RRuulleess::
IIssssuuee ddaattee:: 06.12.2024
CEN Standard EN 15804:2012+A2:2019 serves as core
The Norwegian EPD Foundation PCR VVaalliidd ttoo:: 06.12.2029
NPCR 022:2022 Part B for Roof waterproofing
EEPPDD ssooffttwwaarree::
LCAno EPD generator ID: 707162
1 / 12
GGeenneerraall iinnffoorrmmaattiioonn
PPrroodduucctt:: OOwwnneerr ooff tthhee ddeeccllaarraattiioonn::
Isola Takshingel Premium Rett Isola AS
Contact person: Trond Risberg
Phone: +47 98 89 18 86
e-mail: t.risberg@isola.no
PPrrooggrraamm ooppeerraattoorr:: MMaannuuffaaccttuurreerr::
The Norwegian EPD Foundation Isola AS
Post Box 5250 Majorstuen, 0303 Oslo, Norway
Phone: +47 977 22 020
web: www.epd-norge.no
DDeeccllaarraattiioonn nnuummbbeerr:: PPllaaccee ooff pprroodduuccttiioonn::
Isola AS
NEPD-8335-8004-EN
Prestemoen 9
3946 Porsgrunn, Norway
TThhiiss ddeeccllaarraattiioonn iiss bbaasseedd oonn PPrroodduucctt CCaatteeggoorryy RRuulleess:: MMaannaaggeemmeenntt ssyysstteemm::
CEN Standard EN 15804:2012+A2:2019 serves as core PCR ISO 9001 Certificate No: QSC-6011, ISO 14001:2015
NPCR 022:2022 Part B for Roof waterproofing
SSttaatteemmeenntt ooff lliiaabbiilliittyy:: OOrrggaanniissaattiioonn nnoo::
The owner of the declaration shall be liable for the underlying 928 764 745
information and evidence. EPD Norway shall not be liable with respect
to manufacturer information, life cycle assessment data and
evidences.​
DDeeccllaarreedd uunniitt:: IIssssuuee ddaattee::
1 m2 Isola Takshingel Premium Rett 06.12.2024
DDeeccllaarreedd uunniitt ((ccrraaddllee ttoo ggaattee)) wwiitthh ooppttiioonn:: VVaalliidd ttoo::
A1-A3,A4,A5,C1,C2,C3,C4,D 06.12.2029
YYeeaarr ooff ssttuuddyy::
2023
FFuunnccttiioonnaall uunniitt:: CCoommppaarraabbiilliittyy::
1m² roof covered with Isola Takshingel EPD of construction products may not be comparable if they not
comply with EN 15804 and seen in a building context.
GGeenneerraall iinnffoorrmmaattiioonn oonn vveerriiffiiccaattiioonn ooff EEPPDD ffrroomm EEPPDD ttoooollss:: DDeevveellooppmmeenntt aanndd vveerriiffiiccaattiioonn ooff EEPPDD::
Independent verification of data, other environmental information The declaration is created using EPD tool lca.tools ver EPD2022.03,
and the declaration according to ISO 14025:2010, § 8.1.3 and § 8.1.4. developed by LCA.no. The EPD tool is integrated in the company's
Verification of each EPD is made according to EPD-Norway’s management system, and has been approved by EPD Norway.
guidelines for verification and approval requiring that tools are i) NEPDT19
integrated into the company's environmental management system, ii)
the procedures for use of the EPD tool are approved by EPD-Norway, Developer of EPD: Raquel Flavio
and iii) the process is reviewed annually by an independent third
Reviewer of company-specific input data and EPD: Trond Risberg
party verifier. See Appendix G of EPD-Norway's General Programme
Instructions for further information on EPD tools
VVeerriiffiiccaattiioonn ooff EEPPDD ttooooll:: AApppprroovveedd::
Independent third party verification of the EPD tool, background data
and test-EPD in accordance with EPDNorway's procedures and
guidelines for verification and approval of EPD tools.
Third party verifier:
Elisabet Amat, GREENIZE projects
(no signature required)
2 / 12
PPrroodduucctt::
PPrroodduucctt ddeessccrriippttiioonn::
This is a product specific EPD for Isola Isola Takshingel Premium Rett. Isola Takshingel is an asphalt roofing coating made with a fibreglass core
saturated with polymer-modified bitumen and can be used both on new-bulit buildings and for rehabilitation.
PPrroodduucctt ssppeecciiffiiccaattiioonn
An advanced adhesive system in the sprinkled surface means that adhesion is immediate. The upper part of the back is coated with plastic foil that
provides an antifriction layer and prevents adhesion in the package and to the substrate. Isola Shingel is ideal for use on cold and ventilated roof
constructions.
MMaatteerriiaallss kkgg %%
Additives 0,02 0,20
Bitumen 2,88 24,81
Chemical 0,03 0,28
Polyester film 0,02 0,18
Polypropylene (PP) 0,43 3,74
Raw materials, Mineral 7,91 68,20
Reinforcement 0,30 2,59
Total 11,59 100,00
PPaacckkaaggiinngg kkgg %%
Packaging - Plastic 0,03 16,56
Packaging - Wood 0,13 83,44
Total incl. packaging 11,74 100,00
TTeecchhnniiccaall ddaattaa::
Thickness: 3,2 mm
Dimensional variation: ± 3 mm
External fire performance according to EN 13501-5: Broof (t1), Broof (t2), Broof (t3)
MMaarrkkeett::
EU
RReeffeerreennccee sseerrvviiccee lliiffee,, pprroodduucctt
> 30 years
RReeffeerreennccee sseerrvviiccee lliiffee,, bbuuiillddiinngg
60 years
LLCCAA:: CCaallccuullaattiioonn rruulleess
DDeeccllaarreedd uunniitt::
1 m2 Isola Takshingel Premium Rett
CCuutt--ooffff ccrriitteerriiaa::
All major raw materials and all the essential energy is included. The production processes for raw materials and energy flows with very small
amounts (less than 1%) are not included. These cut-off criteria do not​ apply for hazardous materials and substances.
AAllllooccaattiioonn::
The allocation is made in accordance with the provisions of EN 15804. Incoming energy and water and waste production in-house is allocated
equally among all products through mass allocation. Effects of primary production of recycled materials is allocated to the main product in which
the material was used. The recycling process and transportation of the material is allocated to this analysis. The allocation is made in accordance
with the provisions of EN 15804. Incoming energy and water and waste production in-house is allocated equally among all products through
mass allocation. Effects of primary production of recycled materials is allocated to the main product in which the material was used. The recycling
process and transportation of the material is allocated to this analysis.
DDaattaa qquuaalliittyy::
Specific data for the product composition are provided by the manufacturer. They represent the production of the declared product and were
collected for EPD development in the year of study. Background data is based on registered EPDs according to EN 15804, Ostfold Research
databases, ecoinvent and other LCA databases. The data quality of the raw materials in A1 is presented in the table below.​
Specific data for the product composition are provided by the manufacturer. They represent the production of the declared product and were
collected for EPD development in the year of study. Background data is based on registered EPDs according to EN 15804, Ostfold Research
databases, ecoinvent and other LCA databases. The data quality of the raw materials in A1 is presented in the table below.
3 / 12
MMaatteerriiaallss SSoouurrccee DDaattaa qquuaalliittyy YYeeaarr
Additives ecoinvent 3.6 Database 2019
Bitumen Eurobitume (2019) LCI 2019
Chemical LCA.no Database 2024
Packaging - Plastic ecoinvent 3.6 Database 2019
Packaging - Wood ecoinvent 3.6 Database 2019
Polyester film ecoinvent 3.6 Database 2019
Polypropylene (PP) ecoinvent 3.6 Database 2019
Raw materials, Mineral ecoinvent 3.6 Database 2019
Raw materials, Mineral LCA.no Database 2024
Reinforcement ecoinvent 3.6 Database 2019
4 / 12
SSyysstteemm bboouunnddaarriieess ((XX==iinncclluuddeedd,, MMNNDD==mmoodduullee nnoott ddeeccllaarreedd,, MMNNRR==mmoodduullee nnoott rreelleevvaanntt))
CCoonnssttrruuccttiioonn BBeeyyoonndd tthhee ssyysstteemm
PPrroodduucctt ssttaaggee UUssee ssttaaggee EEnndd ooff lliiffee ssttaaggee
iinnssttaallllaattiioonn ssttaaggee bboouunnddaarriieess
A1 A2 A3 A4 A5 B1 B2 B3 B4 B5 B6 B7 C1 C2 C3 C4 D
X X X X X MND MND MND MND MND MND MND X X X X X
SSyysstteemm bboouunnddaarryy::
AAddddiittiioonnaall tteecchhnniiccaall iinnffoorrmmaattiioonn::
waR slairetam tropsnarT gnirutcafunaM tropsnarT ylbmessA e​sU ecnanetniaM riapeR tnemecalpeR tnemhsibrufeR lanoitarepO ygrene esu lanoitarepO esu retaw -eD noitcurtsnoc noitilomed tropsnarT etsaW gnissecorp lasopsiD -yrevoceR-esueR laitnetop-gnilcyceR
5 / 12
LLCCAA:: SScceennaarriiooss aanndd aaddddiittiioonnaall tteecchhnniiccaall iinnffoorrmmaattiioonn
The following information describe the scenarios in the different modules of the EPD.
The following information describe the scenarios in the different modules of the EPD. The product is produced in A3 and installed manually with
neglectable energy use in A5, assuming a 5% material loss. The packaging waste is treated appropriately. Module C1 is included but assumed to
be zero, since the product contributes minimally to the total environmental load of a building demolition.The product is assumed to be incinerated
with energy recovery in C3. The benefit of substituting energy (heat and electricity) is included in module D.
TTrraannssppoorrtt ffrroomm pprroodduuccttiioonn ppllaaccee ttoo uusseerr CCaappaacciittyy uuttiilliissaattiioonn VVaalluuee
DDiissttaannccee ((kkmm)) FFuueell//EEnneerrggyy CCoonnssuummppttiioonn UUnniitt
((AA44)) ((iinnccll.. rreettuurrnn)) %% ((LLiitteerr//ttoonnnnee))
Truck, EURO 6 (kgkm) 36,7 % 300 0,043 l/tkm 12,90
AAsssseemmbbllyy ((AA55)) UUnniitt VVaalluuee
Material loss (kg) Units/DU 0,05
Waste treatment, packaging, plastic film (LDPE)
kg 0,03
(kg)
Waste treatment, packaging, pallet, EUR wooden
kg 0,13
pallet, single use (kg)
CCaappaacciittyy uuttiilliissaattiioonn VVaalluuee
TTrraannssppoorrtt ttoo wwaassttee pprroocceessssiinngg ((CC22)) DDiissttaannccee ((kkmm)) FFuueell//EEnneerrggyy CCoonnssuummppttiioonn UUnniitt
((iinnccll.. rreettuurrnn)) %% ((LLiitteerr//ttoonnnnee))
Truck, EURO 6 (kgkm) 36,7 % 85 0,043 l/tkm 3,66
WWaassttee pprroocceessssiinngg ((CC33)) UUnniitt VVaalluuee
Waste treatment per kg Bitumen sheet,
kg 10,49
incineration with fly ash extraction (kg)
DDiissppoossaall ((CC44)) UUnniitt VVaalluuee
Landfilling of ashes from incineration of bitumen
kg 3,88
sheet, process per kg ashes and residues (kg)
BBeenneeffiittss aanndd llooaaddss bbeeyyoonndd tthhee ssyysstteemm
UUnniitt VVaalluuee
bboouunnddaarriieess ((DD))
Substitution of electricity, in Norway (MJ) MJ 14,97
Substitution of thermal energy, district heating, in
MJ 226,53
Norway (MJ)
6 / 12
LLCCAA:: RReessuullttss
The LCA results are presented below for the declared unit defined on page 2 of the EPD document.
EEnnvviirroonnmmeennttaall iimmppaacctt
IInnddiiccaattoorr UUnniitt A1-A3 A4 A5 C1 C2 C3 C4 D
GWP-total kg CO2 -eq 4,02E+00 5,14E-01 1,96E-01 0 1,46E-01 2,47E+01 8,62E-02 -1,36E+00
GWP-fossil kg CO2 -eq 4,16E+00 5,14E-01 5,37E-03 0 1,46E-01 2,46E+01 8,62E-02 -1,31E+00
GWP-biogenic kg CO2 -eq -1,43E-01 2,13E-04 1,91E-01 0 6,03E-05 9,15E-04 5,26E-05 -2,71E-03
GWP-luluc kg CO2 -eq 2,36E-03 1,83E-04 1,02E-06 0 5,18E-05 2,28E-04 1,79E-05 -4,52E-02
ODP kg CFC11 -eq 8,02E-07 1,16E-07 6,61E-10 0 3,30E-08 9,62E-08 1,56E-08 -9,57E-02
AP mol H+ -eq 2,29E-02 1,48E-03 2,97E-05 0 4,19E-04 8,07E-03 4,15E-04 -1,08E-02
EP-FreshWater kg P -eq 9,13E-05 4,11E-06 4,47E-08 0 1,16E-06 9,65E-06 1,05E-06 -1,17E-04
EP-Marine kg N -eq 4,69E-03 2,92E-04 1,39E-05 0 8,28E-05 1,97E-03 1,39E-04 -3,54E-03
EP-Terrestial mol N -eq 5,16E-02 3,27E-03 1,34E-04 0 9,26E-04 2,06E-02 1,56E-03 -3,82E-02
POCP kg NMVOC -eq 1,73E-02 1,25E-03 3,51E-05 0 3,55E-04 5,23E-03 4,41E-04 -1,05E-02
ADP-minerals&metals1 kg Sb-eq 9,61E-05 1,42E-05 6,55E-08 0 4,02E-06 4,09E-06 8,49E-07 -1,31E-05
ADP-fossil1 MJ 2,05E+02 7,77E+00 4,80E-02 0 2,20E+00 3,60E+00 1,22E+00 -1,88E+01
WDP1 m3 1,47E+02 7,52E+00 9,02E-02 0 2,13E+00 9,38E+00 6,58E+00 -2,34E+02
GWP-total = Global Warming Potential total; GWP-fossil = Global Warming Potential fossil fuels; GWP-biogenic = Global Warming Potential biogenic; GWP-luluc =
Global Warming Potential land use and land use change; ODP = Depletion potential of the stratospheric ozone layer; AP = Acidification potential, Accumulated
Exceedance; EP-freshwater = Eutrophication potential, fraction of nutrients reaching freshwater end compartment: EP-marine = Eutrophication potential, fraction of
nutrients reaching marine end compartment; EP-terrestrial = Eutrophication potential, Accumulated Exceedance; POCP = Formation potential of tropospheric ozone;
ADP-minerals&metals = Abiotic depletion potential for non-fossil resources; ADP-fossil = Abiotic depletion for fossil resources potential; WDP = Water (user)
deprivation potential, deprivation-weighted water consumption
"Reading example: 9,0 E-03 = 9,0*10-3 = 0,009"
*INA Indicator Not Assessed
1. The results of this environmental impact indicator shall be used with care as the uncertainties on these results are high or as there is limited experienced with the
indicator
RReemmaarrkkss ttoo eennvviirroonnmmeennttaall iimmppaaccttss
7 / 12
AAddddiittiioonnaall eennvviirroonnmmeennttaall iimmppaacctt iinnddiiccaattoorrss
IInnddiiccaattoorr UUnniitt A1-A3 A4 A5 C1 C2 C3 C4 D
PM Disease incidence 7,74E-07 3,15E-08 3,77E-10 0 8,92E-09 4,64E-08 6,46E-09 -6,56E-07
IRP2 kgBq U235 -eq 1,51E-01 3,40E-02 1,81E-04 0 9,63E-03 1,04E-02 5,25E-03 -1,20E-01
ETP-fw1 CTUe 7,03E+01 5,76E+00 5,32E-02 0 1,63E+00 5,73E+00 1,34E+00 -1,02E+02
HTP-c1 CTUh 4,48E-07 0,00E+00 5,00E-12 0 0,00E+00 5,45E-10 5,80E-11 -1,87E-09
HTP-nc1 CTUh 5,16E-07 6,29E-09 2,49E-10 0 1,78E-09 1,65E-08 2,09E-09 -9,79E-08
SQP1 dimensionless 7,02E+01 5,44E+00 3,66E-02 0 1,54E+00 5,62E-01 2,94E+00 -1,26E+02
PM = Particulate Matter emissions; IRP = Ionizing radiation – human health; ETP-fw = Eco toxicity – freshwater; HTP-c = Human toxicity – cancer effects; HTP-nc =
Human toxicity – non cancer effects; SQP = Soil Quality (dimensionless)
"Reading example: 9,0 E-03 = 9,0*10-3 = 0,009"
*INA Indicator Not Assessed
1. The results of this environmental impact indicator shall be used with care as the uncertainties on these results are high or as there is limited experienced with the
indicator
2. This impact category deals mainly with the eventual impact of low dose ionizing radiation on human health of the nuclear fuel cycle. It does not consider effects due
to possible nuclear accidents, occupational exposure nor due to radioactive waste disposal in underground facilities. Potential ionizing radiation from the soil, from
radon and from some construction materials is also not measured by this indicator.
8 / 12
RReessoouurrccee uussee
IInnddiiccaattoorr UUnniitt A1-A3 A4 A5 C1 C2 C3 C4 D
PERE MJ 6,72E+00 1,11E-01 1,02E-03 0 3,15E-02 2,38E-01 4,24E-02 -1,16E+02
PERM MJ 1,80E+00 0,00E+00 -1,75E+00 0 0,00E+00 0,00E+00 0,00E+00 0,00E+00
PERT MJ 8,52E+00 1,11E-01 -1,75E+00 0 3,15E-02 2,38E-01 4,24E-02 -1,16E+02
PENRE MJ 7,13E+01 7,77E+00 4,80E-02 0 2,20E+00 3,60E+00 1,22E+00 -1,88E+01
PENRM MJ 1,34E+02 0,00E+00 -1,06E+00 0 0,00E+00 0,00E+00 0,00E+00 0,00E+00
PENRT MJ 2,06E+02 7,77E+00 -1,01E+00 0 2,20E+00 3,60E+00 1,22E+00 -1,88E+01
SM kg 5,96E-01 0,00E+00 0,00E+00 0 0,00E+00 0,00E+00 0,00E+00 0,00E+00
RSF MJ 1,09E-01 3,98E-03 2,93E-05 0 1,13E-03 6,98E-03 1,08E-03 -2,03E-02
NRSF MJ 5,24E-02 1,42E-02 2,86E-04 0 4,03E-03 0,00E+00 3,70E-02 -6,88E+00
FW m3 6,63E-02 8,31E-04 3,33E-05 0 2,36E-04 1,39E-02 1,11E-03 -1,40E-01
PERE = Use of renewable primary energy excluding renewable primary energy resources used as raw materials; PERM = Use of renewable primary energy resources used
as raw materials; PERT = Total use of renewable primary energy resources; PENRE = Use of non renewable primary energy excluding non-renewable primary energy
resources used as raw materials; PENRM = Use of non renewable primary energy resources used as raw materials; PENRT = Total use of non renewable primary energy
resources; SM = Use of secondary materials; RSF = Use of renewable secondary fuels; NRSF = Use of non-renewable secondary fuels; FW = Net use of fresh water
"Reading example: 9,0 E-03 = 9,0*10-3 = 0,009"
*INA Indicator Not Assessed
9 / 12
EEnndd ooff lliiffee -- WWaassttee
IInnddiiccaattoorr UUnniitt A1-A3 A4 A5 C1 C2 C3 C4 D
HWD kg 9,64E-02 4,01E-04 0,00E+00 0 1,14E-04 0,00E+00 3,72E+00 -8,83E-04
NHWD kg 1,06E+00 3,78E-01 1,51E-01 0 1,07E-01 0,00E+00 4,78E-01 -4,44E-01
RWD kg 1,67E-03 5,29E-05 0,00E+00 0 1,50E-05 0,00E+00 7,44E-06 -9,83E-05
HWD = Hazardous waste disposed; NHWD = Non-hazardous waste disposed; RWD = Radioactive waste disposed
"Reading example: 9,0 E-03 = 9,0*10-3 = 0,009"
*INA Indicator Not Assessed
EEnndd ooff lliiffee -- OOuuttppuutt ffllooww
IInnddiiccaattoorr UUnniitt A1-A3 A4 A5 C1 C2 C3 C4 D
CRU kg 0,00E+00 0,00E+00 0,00E+00 0 0,00E+00 0,00E+00 0,00E+00 0,00E+00
MFR kg 1,80E-02 0,00E+00 1,28E-02 0 0,00E+00 0,00E+00 0,00E+00 0,00E+00
MER kg 4,22E-01 0,00E+00 1,25E-01 0 0,00E+00 1,05E+01 0,00E+00 0,00E+00
EEE MJ 2,52E-01 0,00E+00 8,69E-02 0 0,00E+00 1,50E+01 0,00E+00 0,00E+00
EET MJ 3,82E+00 0,00E+00 1,32E+00 0 0,00E+00 2,27E+02 0,00E+00 0,00E+00
CRU = Components for re-use; MFR = Materials for recycling; MER = Materials for energy recovery; EEE = Exported energy electrical; EET = Exported energy thermal
"Reading example: 9,0 E-03 = 9,0*10-3 = 0,009"
*INA Indicator Not Assessed
BBiiooggeenniicc CCaarrbboonn CCoonntteenntt
IInnddiiccaattoorr UUnniitt AAtt tthhee ffaaccttoorryy ggaattee
Biogenic carbon content in product kg C 0,00E+00
Biogenic carbon content in accompanying packaging kg C 5,37E-02
Note: 1 kg biogenic carbon is equivalent to 44/12 kg CO2
10 / 12
AAddddiittiioonnaall rreeqquuiirreemmeennttss
GGrreeeennhhoouussee ggaass eemmiissssiioonnss ffrroomm tthhee uussee ooff eelleeccttrriicciittyy iinn tthhee mmaannuuffaaccttuurriinngg pphhaassee
National production mix from import, low voltage (production of transmission lines, in addition to direct emissions and losses in grid) of applied
electricity for the manufacturing process (A3).
EElleeccttrriicciittyy mmiixx SSoouurrccee AAmmoouunntt UUnniitt
Electricity, Norway (kWh) ecoinvent 3.6 24,33 g CO2-eq/kWh
DDaannggeerroouuss ssuubbssttaanncceess
The product contains no substances given by the REACH Candidate list.
IInnddoooorr eennvviirroonnmmeenntt
AAddddiittiioonnaall EEnnvviirroonnmmeennttaall IInnffoorrmmaattiioonn
AAddddiittiioonnaall eennvviirroonnmmeennttaall iimmppaacctt iinnddiiccaattoorrss rreeqquuiirreedd iinn NNPPCCRR PPaarrtt AA ffoorr ccoonnssttrruuccttiioonn pprroodduuccttss
IInnddiiccaattoorr UUnniitt A1-A3 A4 A5 C1 C2 C3 C4 D
GWPIOBC kg CO2 -eq 4,21E+00 5,14E-01 5,37E-03 0 1,46E-01 2,47E+01 8,62E-02 -1,34E+00
GWP-IOBC: Global warming potential calculated according to the principle of instantaneous oxidation. In order to increase the transparency of biogenic carbon​
contribution to climate impact, the indicator GWP-IOBC is required as it declares climate impacts calculated according to the principle of instantaneous oxidation.​
GWP-IOBC is also referred to as GWP-GHG in context to Swedish public procurement legislation.
11 / 12
BBiibblliiooggrraapphhyy
ISO 14025:2010 Environmental labels and declarations - Type III environmental declarations - Principles and procedures.
ISO 14044:2006 Environmental management - Life cycle assessment - Requirements and guidelines.
EN 15804:2012+A2:2019 Environmental product declaration - Core rules for the product category of construction products.
ISO 21930:2017 Sustainability in buildings and civil engineering works - Core rules for environmental product declarations of construction
products.
ecoinvent v3, Allocation, cut-off by classification, Swiss Centre of Life Cycle Inventories.
Iversen et al., (2018) eEPD v3.0 - Background information for EPD generator system. LCA.no report number 04.18.
Ruttenborg et al., (2023) EPD generator for NPCR022:2022 Part B for Roof waterproofing - Background information for EPD generator application
and LCA data, LCA.no report number 10.23
NPCR Part A: Construction products and services. Ver. 2.0. March 2021, EPD-Norge.
NPCR 022 Part B for Roof waterproofing. Ver. 2.0 March 2022, EPD-Norge.
PPrrooggrraamm ooppeerraattoorr aanndd ppuubblliisshheerr Phone: +47 977 22 020
The Norwegian EPD Foundation e-mail: post@epd-norge.no
Post Box 5250 Majorstuen, 0303 Oslo, Norway web: www.epd-norge.no
OOwwnneerr ooff tthhee ddeeccllaarraattiioonn:: Phone: +47 98 89 18 86
Isola AS e-mail: t.risberg@isola.no
Prestemoen 9, 3946 Porsgrunn, Norway web: www.isola.no
AAuutthhoorr ooff tthhee LLiiffee CCyyccllee AAsssseessssmmeenntt Phone: +47 916 50 916
LCA.no AS e-mail: post@lca.no
Dokka 6A, 1671 Kråkerøy, Norway web: www.lca.no
DDeevveellooppeerr ooff EEPPDD ggeenneerraattoorr Phone: +47 916 50 916
LCA.no AS e-mail: post@lca.no
Dokka 6A, 1671 Kråkerøy, Norway web: www.lca.no
ECO Platform web: www.eco-platform.org
ECO Portal web: ECO Portal
12 / 12
