ver1 2015
ENVIRONMENTAL PRODUCT DECLARATION
in accordance with ISO 14025, ISO 21930 and EN 15804
Owner of the declaration: Jotun A /S
Program operator: T he Norwegian EP D Foundation
Publisher: T he Norwegian EP D Foundation
Declaration number: NEPD-2210-1017-EN
Registration number: NEPD-2210-1017-EN
ECO Platform reference number: -
Issue date: 25.05.2020
Valid to: 25.05.2025
Fenomastic Hygiene Emulsion Matt, El-Mohandes Jotun S.A.E. (Egypt)
Jotun A/S
www.epd-norge.no
NEPD-2210-1017-EN Fenomastic Hygiene Emulsion Matt, El-Mohandes Jotun S.A.E. (Egypt) 1 / 8
General information
Product: Owner of the declaration:
Fenomastic Hygiene Emulsion Matt, El-Mohandes Jotun S.A.E.
Jotun A/S
(Egypt)
Contact person: Anne Lill Gade
Phone: +47 33 45 70 00
e-mail: anne.lill.gade@jotun.no
Program operator: Manufacturer:
T he Norwegian EP D Foundation Jotun A/S
P b. 5250 M ajorstuen, 0303 O slo
P hone: +47 97722020
e-mail: post@epd-norge.no
Declaration number: Place of production:
NEPD-2210-1017-EN El-Mohandes Jotun S.A.E.
Industrial Area, Ismailia
Egypt
ECO Platform reference number: Management system:
ISO 9001:2008 Certificate nr: 0044915-00, ISO 14001:2004
Certificate nr 0044914-00, OHSAS 18001:2007 Certificate nr:
0044916-00.
This declaration is based on Product Category Rules: Organisation no:
923 248 579
CEN Standard EN 15804:2012+A1:2013 serves as core PCR.
Product descriptions and scenarios are based on IBU PCR Part B
for coatings with organic binders. This also applies for inorganic
coatings.
Statement of liability: Issue date: 25.05.2020
The owner of the declaration shall be liable for the underlying
information and evidence. EPD Norway shall not be liable with Valid to: 25.05.2025
respect to manufacturer information, life cycle assessment data
and evidences.
Declared unit: Year of study:
1 kg Fenomastic Hygiene Emulsion Matt, El-Mohandes Jotun S.A.E.
2020
(Egypt)
Declared unit with option: Comparability:
EPD of construction products may not be comparable if they not
A1,A2,A3
comply with EN 15804 and seen in a building context.
Functional unit: Author of the Life Cycle Assessment:
The declaration is developed using eEPD v4.0 from LCA.no
Approval:
Company specific data are:
Collected/registered by: Ken Gudvangen
Internal verification by: Cleo Alves Otterbech
Verification: Approved:
Independent verification of data, other environmental information
and the declaration according to ISO14025:2010, § 8.1.3 and §
8.1.4
External
Third party verifier:
Sign Sign
Senior Research Scientist, Anne Rønning
(Independent verifier approved by EPD Norway)
NEPD-2210-1017-EN Fenomastic Hygiene Emulsion Matt, El-Mohandes Jotun S.A.E. (Egypt) 2 / 8
Product
Product description: Technical data:
Fenomastic Hygiene Emulsion Matt is a superior quality emulsion TDS Specific gravity: 1.43
paint, designed for interior surfaces. It is based on pure acrylic SDS Density: 1.261 to 1.448 g/cm³
emulsion and is a specially designed product to offer resistance Solids by volume: 33 ± 2 volume%
against 22 different varieties of bacteria and fungus.
Film thickness per coat:
Fenomastic Hygiene Emulsion Matt offers good flow, hiding power, Dry film thickness: 33 - 50 µm
incan anti bacterial and colour retention properties. It has very good Wet film thickness: 100 - 150 µm
opacity, outstanding washability and leveling, thereby creating a Theoretical spreading rate: 10 - 6.6 m²/l
high-class finish. The product provides smooth durable and washable
matt finish. It is free from harmful chemicals like APEO and The most representative and worst case formulation produced at the
formaldehyde. Heavy Metals are not used as active ingredients. manufacturing site is chosen for this EPD. For products with a
selection of colours, this will be the formulation with the highest
The declared product has low VOC which ensures good indoor air content of titanium dioxide.
quality and is strongly recommended for interiors of hospitals, hotels,
schools, wash rooms, kitchens, living rooms etc. The product packaging is based on an average sized metal
packaging, including secondary packaging such as pallets and
Product specification
plastic wrapping.
For information on Green Building Standard credits, see "Additional
Information" on page 4. For safety, health and environmental conditions, see the Safety Data
Sheet for the declared product on www.jotun.com.
The material composition of the declared mixed product is given
below: For information on technical data, application and use of the product,
Materials % see the Technical Data Sheet for the declared product on
www.jotun.com.
Water 25-50
Filler 10-25 Market:
Titanium dioxide 10-25 Global. Transport to market is not included in this EPD.
Binder 5-10
Reference service life, product
Solvent 1-3
The reference service life of the product is highly dependent on the
Additive 0.3-1 conditions of use.
Biocide 0.1-0.3 Estimated service life, object
Pigment <0.1
The coated object is not declared.
LCA: Calculation rules
Declared unit: Allocation:
1 kg Fenomastic Hygiene Emulsion Matt, El-Mohandes Jotun S.A.E. The allocation is made in accordance with the provisions of EN
(Egypt) 15804. Incoming energy, water and waste production in-house is
primarily allocated equally among all products through mass
Cut-off criteria:
allocation. Specific allocation was performed for certain waste flows
All major raw materials and essential energy is included. The according to information provided by the site manager. VOC
production process for raw materials and energy flows with very small emissions have been allocated entirely to the production of solvent
amounts (less than 0.1 % dry matter) are not included. In total, more based paints. Effects of primary production of recycled materials is
than 99% of the material input is included. These cut-off criteria do allocated to the main product in which the material was used. The
not apply for non-energy related emissions (such as wastes, recycling process and transportation of the material is allocated to
hazardous materials and substances). this analysis.
Data quality:
The CEPE database is used as basis for the raw material composition. Specific data for the product composition and raw material amounts
has been provided by the manufacturer and represents the production of the declared product. Production site data was collected in 2015.
Representative data from ecoinvent v3.2 was used for other processes. The data quality for the material input in A1 is presented in tabular
form.
Materials Source Data quality Year
Additives CEPE RM Database v3.0 Database 2016
Binders and Resins CEPE RM Database v3.0 Database 2016
Others CEPE RM Database v3.0 Database 2016
Pigments and Fillers CEPE RM Database v3.0 Database 2016
Solvents CEPE RM Database v3.0 Database 2016
Packaging Østfoldforskning Database 2017
NEPD-2210-1017-EN Fenomastic Hygiene Emulsion Matt, El-Mohandes Jotun S.A.E. (Egypt) 3 / 8
System boundary:
The flowchart in the figure below illustrates the system boundaries for the analysis, in accordance with the modular principle of EN 15804.
The analysis is a cradle-to-gate (A1 - A3) study.
Additional information:
The declared product contributes to Green Building Standard credits by meeting the following specific requirements:
LEED®v4.1 (2019):
EQ credit: Low-emitting materials.
- VOC content for Interior matt walls and ceilings (Gloss <25 at 60°) (30 g/l) (EU Directive 2004/42/CE) and emission range less or equal
to 0.5 mg/m3 (CDPH method 1.2)
LEED®v4 (2013)/ LEED®v4.1 (2019):
EQ credit: Low-emitting materials
- VOC content for Flat coatings (50 g/l) (CARB(SCM)2007) and emission less or equal to 0.5 mg/m3 (CDPH method 1.2 (2017))
MR credit: Building product disclosure and optimization
- Material Ingredients, Option 2: Material Ingredient Optimization, International Alternative Compliance Path - REACH optimization: Fully
inventoried chemical ingredients to 100 ppm and not containing substances on the REACH Authorization list – Annex XIV, the Restriction
list – Annex XVII and the SVHC candidate list.
- Environmental Product Declarations. Product-specific Type III EPD (ISO 14025;21930, EN 15804) for El-Mohandes Jotun S.A.E.
(Egypt).
BREEAM International (2016):
- Hea 02: VOC emission ((ISO 16000-series (2006) or CDPH method 1.2 (2017)) and the VOC content for Interior matt walls and ceilings
(10 g/l)
- Mat 01: Product-specific Type III EPD (ISO 14025;21930, EN 15804) for El-Mohandes Jotun S.A.E. (Egypt).
Additional certificates and approvals may be available on request.
NEPD-2210-1017-EN Fenomastic Hygiene Emulsion Matt, El-Mohandes Jotun S.A.E. (Egypt) 4 / 8
LCA: Scenarios and additional technical information
The following information describe the scenarios in the different modules of the EPD.
This is a cradle to gate (A1-A3) EPD with no declared modules after the factory gate. Transport from place of production to user (A4) has to
be calculated by the user.
NEPD-2210-1017-EN Fenomastic Hygiene Emulsion Matt, El-Mohandes Jotun S.A.E. (Egypt) 5 / 8
LCA: Results
System boundaries (X=included, MND=module not declared, MNR=module not relevant)
Construction Beyond the
Product stage installation User stage End of life stage . system
stage bondaries
A1 A2 A3 A4 A5 B1 B2 B3 B4 B5 B6 B7 C1 C2 C3 C4 . D
X X X MND MND MND MND MND MND MND MND MND MND MND MND MND . MND
Environmental impact
Parameter Unit A1 A2 A3
GWP kg CO 2 -eq 2,37E+00 1,01E-01 5,13E-02
ODP kg CFC11 -eq 2,05E-07 1,89E-08 7,14E-09
POCP kg C 2H 4-eq 1,26E-03 3,73E-05 7,11E-04
AP kg SO 2 -eq 1,60E-02 1,12E-03 3,51E-04
EP kg PO 3- -eq 3,57E-03 1,59E-04 3,57E-05
4
ADPM kg Sb -eq 2,82E-05 1,24E-07 2,64E-08
ADPE MJ 3,06E+01 1,60E+00 7,87E-01
GWP Global warming potential; ODP Depletion potential of the stratospheric ozone layer; POCP Formation potential of tropospheric photochemical
oxidants; AP Acidification potential of land and water; EP Eutrophication potential; ADPM Abiotic depletion potential for non fossil resources; ADPE
Abiotic depletion potential for fossil resources
Reading example: 9,0 E-03 = 9,0*10-3 = 0,009
*INA Indicator Not Assessed
waR slairetam tropsnarT gnirutcafunaM tropsnarT ylbmessA esU ecnanetniaM riapeR tnemecalpeR tnemhsibrufeR lanoitarepO ygrene esu lanoitarepO esu
retaw
-eD noitcurtsnoc noitilomed tropsnarT etsaW gnissecorp lasopsiD -yrevoceR-esueR -gnilcyceR laitnetop
NEPD-2210-1017-EN Fenomastic Hygiene Emulsion Matt, El-Mohandes Jotun S.A.E. (Egypt) 6 / 8
Resource use
Parameter Unit A1 A2 A3
RPEE MJ 2,40E+00 2,67E-02 2,60E-03
RPEM MJ 5,09E-01 6,65E-03 4,67E-04
TPE MJ 2,91E+00 3,33E-02 3,06E-03
NRPE MJ 3,40E+01 1,63E+00 7,93E-01
NRPM MJ 0,00E+00 0,00E+00 0,00E+00
TRPE MJ 3,40E+01 1,63E+00 7,93E-01
SM kg 0,00E+00 0,00E+00 0,00E+00
RSF MJ 0,00E+00 0,00E+00 0,00E+00
NRSF MJ 0,00E+00 0,00E+00 0,00E+00
W m3 2,85E-01 3,12E-04 1,23E-04
RPEE Renewable primary energy resources used as energy carrier; RPEM Renewable primary energy resources used as raw materials; TPE Total use
of renewable primary energy resources; NRPE Non renewable primary energy resources used as energy carrier; NRPM Non renewable primary energy
resources used as materials; TRPE Total use of non renewable primary energy resources; SM Use of secondary materials; RSF Use of renewable
secondary fuels; NRSF Use of non renewable secondary fuels; W Use of net fresh water
Reading example: 9,0 E-03 = 9,0*10-3 = 0,009
*INA Indicator Not Assessed
End of life - Waste
Parameter Unit A1 A2 A3
HW kg 4,26E-05 8,72E-07 1,84E-04
NHW kg 1,60E+00 9,55E-02 2,30E-03
RW kg INA* INA* INA*
HW Hazardous waste disposed; NHW Non hazardous waste disposed; RW Radioactive waste disposed
Reading example: 9,0 E-03 = 9,0*10-3 = 0,009
*INA Indicator Not Assessed
End of life - Output flow
Parameter Unit A1 A2 A3
CR kg 0,00E+00 0,00E+00 0,00E+00
MR kg 0,00E+00 0,00E+00 1,13E-05
MER kg 0,00E+00 0,00E+00 2,81E-05
EEE MJ INA* INA* INA*
ETE MJ INA* INA* INA*
CR Components for reuse; MR Materials for recycling; MER Materials for energy recovery; EEE Exported electric energy; ETE Exported thermal
energy
Reading example: 9,0 E-03 = 9,0*10-3 = 0,009
*INA Indicator Not Assessed
NEPD-2210-1017-EN Fenomastic Hygiene Emulsion Matt, El-Mohandes Jotun S.A.E. (Egypt) 7 / 8
Additional requirements
Greenhouse gas emissions from the use of electricity in the manufacturing phase
National production mix from import, low voltage (production of transmission lines, in addition to direct emissions and losses in grid) of
applied electricity for the manufacturing process (A3).
Electricity mix Data source Amount Unit
Electricity, Egypt (kWh) ecoinvent 3.3 Alloc Rec 1113,82 g CO2-ekv/kWh
Dangerous substances
The product contains no substances given by the REACH Candidate list.
Indoor environment
The declared product is emission tested by RISE Research Institutes of Sweden/SP Technical Research Institute of Sweden or Eurofins in
accordance with California Department of Public Health (CDPH) Standard Method v1.1–2010.
Bibliography
ISO 14025:2010 Environmental labels and declarations - Type III environmental declarations - Principles and procedures.
ISO 14044:2006 Environmental management - Life cycle assessment - Requirements and guidelines.
EN 15804:2012+A1:2013 Environmental product declaration - Core rules for the product category of construction products.
ISO 21930:2017 Sustainability in buildings and civil engineering works - Core rules for environmental product declarations of construction
products.
IBU PCR Part B: Requirements on the EPD for Coatings with organic binders. v1.4, September 2016.
Vold et al (2017). EPD and LCA tool for Jotun - Technical description and background information, OR 01.17, Ostfold Research, Fredrikstad
2017.
CEPE v3.0 Raw materials LCI database for the European coatings and printing ink industries, May 2016.
ecoinvent v3.2 Alloc Rec, Swiss Centre of Life Cycle Inventories.
BREEAM International(2016):BREEAM InternationalNewConstruction Technical Manual. SD233-2.0:2017
CARB SCM (2007). California Air Resources Board (ARB) Suggested Control Measure for Architectural Coatings
CDPH method 1.1 (2010)/1.2 (2017): Standard method for the testing and evaluation of volatile organic chemical emissions from indoor
sources. California Department of Public Health
EU Directive 2004/42/CE: The limitation of emissions of volatile organic compounds due to the use of organic solvents in certain paints and
varnishes and vehicle refinishing products
ISO 16000-series of indoor air standards for VOCs sampling and determination, i.e. 3, 6(2011); 9, 10, 11(2006)
LEED® v4.1 (2019): LEED® v4.1 for Building design and construction, U.S. Green Building Council®
LEED® v4(2013): LEED® v4 for Building design and construction, U.S. Green Building Council®
REACH (2006): Regulation (EC) No 1907/2006 of the European Parliament and of the Council of 18 December 2006. REACH Authorization
list – Annex XIV, the Restriction list – Annex XVII and the SVHC candidate list
Program operator and publisher Phone: +47 97722020
The Norwegian EPD Foundation
Post Box 5250 Majorstuen, 0303 Oslo e-mail: post@epd-norge.no
0303 Oslo Norway web: www.epd-norge.no
Owner of the declaration Phone: +47 33 45 70 00
Jotun A/S Fax:
Hystadveien 167 e-mail: anne.lill.gade@jotun.no
3209 Sandefjord web: www.jotun.no
Author of the Life Cycle Assessment Phone: +47 69 35 11 00
Østfoldforskning AS Fax: +47 69 34 24 94
Stadion 4 e-mail:
1671 Kråkerøy web: www.ostfoldforskning.no
Developer of EPD generator Phone: +47 916 50 916
LCA.no AS
Dokka 1C e-mail: post@lca.no
1671 Kråkerøy web: www.lca.no
NEPD-2210-1017-EN Fenomastic Hygiene Emulsion Matt, El-Mohandes Jotun S.A.E. (Egypt) 8 / 8
