Environmental product declaration
in accordance with ISO 14025 and EN 15804+A2
TROX X-CUBE
Owner of the declaration: Program operator:
TROX Group The Norwegian EPD Foundation
Product: Declaration number:
TROX X-CUBE
NEPD-8579-8242-EN
Declared unit:
1 pcs Registration number:
This declaration is based on Product Category Rules: NEPD-8579-8242-EN
CEN Standard EN 15804:2012+A2:2019 serves as core
Issue date: 20.12.2024
PCR
The Norwegian EPD Foundation NPCR 030:2021 Part B for ventilation components Valid to: 20.12.2029
EPD software:
LCAno EPD generator ID: 304359
1 / 12
General information
Product Owner of the declaration:
TROX X-CUBE TROX Group
Contact person: Alina Buchner
Phone: +49 2845 2020
e-mail: productsustainability-de@troxgroup.com
Program operator: Manufacturer:
The Norwegian EPD Foundation TROX Group
Post Box 5250 Majorstuen, 0303 Oslo, Norway Heinrich-Trox-Platz 1
Phone: +47 977 22 020 47506 Neukirchen-Vluyn, Germany
web: www.epd-norge.no
Declaration number: Place of production:
TROX GmbH - Werk Anholt
NEPD-8579-8242-EN
Gendringer Str. 85
46419 Isselburg, Germany
This declaration is based on Product Category Rules: Management system:
CEN Standard EN 15804:2012+A2:2019 serves as core PCR ISO 9001, ISO 14001:2015, ISO 50001:2018
NPCR 030:2021 Part B for ventilation components
Statement of liability: Organisation no:
The owner of the declaration shall be liable for the underlying DE 120250070
information and evidence. EPD Norway shall not be liable with respect
to manufacturer information, life cycle assessment data and
evidences.​
Declared unit: Issue date:
1 pcs TROX X-CUBE 20.12.2024
Declared unit with option: Valid to:
A1-A3,A4,C1,C2,C3,C4,D 20.12.2029
Year of study:
2023
Functional unit: Comparability:
EPD of construction products may not be comparable if they not
comply with EN 15804 and seen in a building context.
General information on verification of EPD from EPD tools: Development and verification of EPD:
Independent verification of data, other environmental information The declaration is created using EPD tool lca.tools ver EPD2022.03,
and the declaration according to ISO 14025:2010, § 8.1.3 and § 8.1.4. developed by LCA.no. The EPD tool is integrated in the company's
Verification of each EPD is made according to EPD-Norway’s management system and has been approved by EPD Norway.
guidelines for verification and approval requiring that tools are i)
integrated into the company's environmental management system, ii) Developer of EPD: Janik Horst
the procedures for use of the EPD tool are approved by EPD-Norway,
Reviewer of company-specific input data and EPD:​ Alina Buchner
and iii) the process is reviewed annually by an independent third
party verifier. See Appendix G of EPD-Norway's General Programme
Instructions for further information on EPD tools
Verification of EPD tool: Approved:
Independent third party verification of the EPD tool, background data
and test-EPD in accordance with EPDNorway's procedures and
guidelines for verification and approval of EPD tools.
Third party verifier:
Alexander Borg, Asplan Viak AS
(no signature required)
2 / 12
Product
Product description:
The TROX X-CUBE is an air handling unit and is used only for the treatment and conditioning of air, i.e. for the ventilation of rooms and entire
buildings, for filtering, heating, cooling, for heat recovery as well as for humidifying and / or dehumidifying air.
Product specification
The X-CUBE units are tailor-made air handling units that can be used for all air treatment processes. X-CUBE units are available as supply or
extract air units, or as a combination of both, arranged side by side or on top of each other.
In addition to a particularly high-quality basic version, a special hygienic variant in accordance with DIN 1946 Part 4 and a weatherproof variant
for outdoor installation are also available.
Each X-CUBE unit is configured according to the customer's individual project-specific requirements.
The volume flow of the calculated device is 30,000 m³/h for supply and extract air. The type designation is supply air 5020/return air 5020.
Materials kg %
Adhesive 8,65 0,16
Adhesive and sealant 5,95 0,11
Electronic - LED chip 3,20 0,06
Electronic - Unspecified 733,20 13,82
Filter, mineral based 35,09 0,66
Glass fibre reinforced plastic,
10,57 0,20
polyamide
Insulation 3,23 0,06
Insulation, Mineral based 385,74 7,27
Metal - Galvanized Steel 2378,73 44,82
Plastic - Acrylonitrile butadiene
178,06 3,35
styrene (ABS)
Plastic - Polybutylene terephthalate
0,11 0,00
(PBT)
Plastic - Polyethylene 0,14 0,00
Plastic - Polyoxymethylene (POM) 0,02 0,00
Plastic - Polypropylene (PP) 2,30 0,04
Plastic - Polystyrene (PS) 34,47 0,65
Plastic - Polyvinyl chloride (PVC) 0,64 0,01
Powder coating 44,13 0,83
Rubber, synthetic 4,11 0,08
Metal - Aluminium 7,84 0,15
Metal - Copper 472,02 8,89
Metal - Stainless steel 983,98 18,54
Metal - Steel 15,06 0,28
Total 5307,21 100,00
Packaging kg %
Packaging - Pallet 20,00 95,78
Packaging - Plastic 0,16 0,75
Packaging - Polystyrene 0,20 0,94
Packaging - Recycled cardboard 0,53 2,53
Total incl. packaging 5328,09 100,00
Technical data:
Limits of the air handling unit:
Volume flow: from 1.200 to approx. 100.000 m³/h (0,3 to 28 m³/s)
Operating temperature: -30 to +50 °C
Variants: 96 sizes
Heat recovery: can be equipped with a rotary heat exchanger, a plate heat exchanger or a RAC system
The product configuration and technical data can be found in the project-specific data sheet.
Market:
Europe.
Reference service life, product
20 years.
Reference service life, building or construction works
60 years.
LCA: Calculation rules
Declared unit:
3 / 12
1 pcs TROX X-CUBE
Cut-off criteria:
All major raw materials and all the essential energy is included. The production processes for raw materials and energy flows with very small
amounts (less than 1%) are not included. These cut-off criteria do not​ apply for hazardous materials and substances.
Allocation:
The allocation is made in accordance with the provisions of EN 15804. Energy, water and waste production in-house is allocated equally among all
products through mass allocation. Effects of primary production of recycled materials is allocated to the main product in which the material was
used. The recycling process and transportation of the material is allocated to this analysis.
Data quality:
Specific data for the product composition are provided by the manufacturer. The data represent the production of the declared product and were
collected for EPD development in the year of study. Background data is based on EPDs according to EN 15804 and different LCA databases. The
data quality of the raw materials in A1 is presented in the table below.
Materials Source Data quality Year
Adhesive Modified ecoinvent 3.6 Database 2019
Adhesive and sealant ecoinvent 3.6 Database 2019
Electronic - LED chip ecoinvent 3.6 Database 2019
Electronic - Unspecified ecoinvent 3.6 Database 2019
Filter, mineral based ecoinvent 3.6 Database 2019
Glass fibre reinforced plastic, polyamide Modified ecoinvent 3.6 Database 2019
Insulation EPD-ARM-20200219-IBB1-DE EPD 2020
Insulation, Mineral based ecoinvent 3.6 Database 2019
Metal - Aluminium ecoinvent 3.6 Database 2019
Metal - Copper ecoinvent 3.6 Database 2019
Metal - Galvanized Steel ecoinvent 3.6 Database 2019
Metal - Galvanized Steel ecoinvent 3.6 Database 2020
Metal - Galvanized Steel Supplier EPD 2023
Metal - Stainless steel ecoinvent 3.6 Database 2019
Metal - Stainless steel EPD-AWU-20230569-CBA1-EN EPD 2023
Metal - Steel ecoinvent 3.6 Database 2019
Packaging - Pallet ecoinvent 3.6 Database 2019
Packaging - Plastic ecoinvent 3.6 Database 2019
Packaging - Polystyrene ecoinvent 3.6 Database 2019
Packaging - Recycled cardboard Modified ecoinvent 3.6 Database 2019
Plastic - Acrylonitrile butadiene styrene (ABS) ecoinvent 3.6 Database 2019
Plastic - Polybutylene terephthalate (PBT) ecoinvent 3.6 Database 2019
Plastic - Polyethylene ecoinvent 3.6 Database 2019
Plastic - Polyoxymethylene (POM) ecoinvent 3.6 Database 2019
Plastic - Polypropylene (PP) ecoinvent 3.6 Database 2019
Plastic - Polystyrene (PS) ecoinvent 3.6 Database 2019
Plastic - Polyvinyl chloride (PVC) ecoinvent 3.6 Database 2019
Powder coating ecoinvent 3.6 Database 2019
Rubber, synthetic ecoinvent 3.6 Database 2019
4 / 12
System boundaries (X=included, MND=module not declared, MNR=module not relevant)
Construction Beyond the system
Product stage Use stage End of life stage
installation stage boundaries
A1 A2 A3 A4 A5 B1 B2 B3 B4 B5 B6 B7 C1 C2 C3 C4 D
X X X X MND MND MND MND MND MND MND MND X X X X X
System boundary:
Additional technical information:
waR slairetam tropsnarT gnirutcafunaM tropsnarT ylbmessA e​sU ecnanetniaM riapeR tnemecalpeR tnemhsibrufeR lanoitarepO ygrene esu lanoitarepO esu retaw -eD noitcurtsnoc noitilomed tropsnarT etsaW gnissecorp lasopsiD -yrevoceR-esueR laitnetop-gnilcyceR
5 / 12
LCA: Scenarios and additional technical information
The following information describe the scenarios in the different modules of the EPD.
Capacity utilisation Value
Transport from production place to user (A4) Distance (km) Fuel/Energy Consumption Unit
(incl. return) % (Liter/tonne)
Truck, 16-32 tonnes, EURO 6 (km) 36,7 % 800 0,043 l/tkm 34,40
De-construction demolition (C1) Unit Value
Demolition of building per kg of ventilation
kg 5307,21
product (kg)
Capacity utilisation Value
Transport to waste processing (C2) Distance (km) Fuel/Energy Consumption Unit
(incl. return) % (Liter/tonne)
Truck, 16-32 tonnes, EURO 6 (km) 36,7 % 50 0,043 l/tkm 2,15
Waste processing (C3) Unit Value
Materials to recycling (kg) kg 3095,24
Waste treatment per kg Rubber, municipal
kg 2,054
incineration with fly ash extraction (kg)
Waste treatment per kg Hazardous waste,
kg 29,36
incineration (kg)
Waste treatment per kg Plastics, incineration (kg) kg 98,20
Waste treatment per kg Polypropylene (PP),
kg 0,19
incineration (kg)
Waste treatment per kg Electronic scrap,
kg 736,40
incineration (kg)
Waste treatment per kg Polyvinylchloride (PVC),
kg 0,0010
incineration with fly ash extraction (kg)
Disposal (C4) Unit Value
Waste, scrap steel, to landfill (kg) kg 294,57
Landfilling of ashes from incineration of Rubber,
kg 0,10
municipal incineration with fly ash extraction (kg)
Waste, plastic, mixture, to landfill (kg) kg 100,45
Landfilling of ashes from incineration per kg
kg 5,54
Hazardous waste, from incineration (kg)
Waste, hazardous waste, to landfill (kg) kg 29,36
Waste, mineral wool, to landfil (kg) kg 162,43
Waste treatment per kg Copper slag, to landfill,
kg 47,20
residual material landfill (kg)
Landfilling of ashes from incineration of Plastics,
kg 2,31
process per kg ashes and residues (kg)
Waste, aluminium, to landfill (kg) kg 1,39
Landfilling of ashes from incineration of
Polypropylene (PP), process per kg ashes and kg 0,0057
residues (kg)
Landfilling of ashes from incineration of
Electronic scrap, process of ashes and residues kg 516,73
(kg)
Substitution of primary steel with net scrap (kg) kg 0,48
Landfilling of ashes from incineration of
Polyvinylchloride (PVC), process per kg ashes and kg 0,00015
residues (kg)
Benefits and loads beyond the system
Unit Value
boundaries (D)
Substitution of primary steel with net scrap (kg) kg 1006,43
Substitution of thermal energy, district heating
MJ 48,36
(MJ)
Substitution of electricity (MJ) MJ 3,19
Substitution of primary copper with net scrap (kg) kg 354,053
Substitution of primary aluminium with net scrap
kg 7,089
(kg)
6 / 12
LCA: Results
The LCA results are presented below for the declared unit defined on page 2 of the EPD document.
Environmental impact
Indicator Unit A1-A3 A4 C1 C2 C3 C4 D
GWP-total kg CO2 -eq 3,50E+04 6,97E+02 7,00E+00 4,35E+01 1,12E+03 8,69E+01 -2,21E+03
GWP-fossil kg CO2 -eq 3,46E+04 6,96E+02 7,00E+00 4,35E+01 1,12E+03 8,67E+01 -2,20E+03
GWP-biogenic kg CO2 -eq 3,53E+02 2,88E-01 1,31E-03 1,80E-02 2,80E-01 1,04E-01 -4,94E+00
GWP-luluc kg CO2 -eq 4,04E+01 2,48E-01 5,52E-04 1,55E-02 4,61E-02 8,02E-02 -2,68E+00
ODP kg CFC11 -eq 2,66E-03 1,58E-04 1,51E-06 9,86E-06 1,30E-05 5,30E-06 -3,35E-02
AP mol H+ -eq 3,64E+02 2,00E+00 7,32E-02 1,25E-01 4,21E-01 1,91E-01 -1,49E+02
EP-FreshWater kg P -eq 3,37E+00 5,56E-03 2,55E-05 3,48E-04 2,62E-03 1,07E-03 -1,04E+00
EP-Marine kg N -eq 4,30E+01 3,96E-01 3,23E-02 2,47E-02 1,54E-01 6,48E-02 -7,22E+00
EP-Terrestial mol N -eq 7,16E+02 4,43E+00 3,55E-01 2,77E-01 1,59E+00 5,65E-01 -1,05E+02
POCP kg NMVOC -eq 1,59E+02 1,70E+00 9,75E-02 1,06E-01 4,01E-01 1,73E-01 -3,13E+01
ADP-minerals&metals1 kg Sb-eq 2,85E+02 1,92E-02 1,07E-05 1,20E-03 6,17E-04 3,48E-04 -8,18E-01
ADP-fossil1 MJ 4,81E+05 1,05E+04 9,63E+01 6,58E+02 6,79E+02 5,00E+02 -1,92E+04
WDP1 m3 1,73E+06 1,02E+04 2,05E+01 6,36E+02 2,21E+03 1,55E+03 7,72E+04
GWP-total = Global Warming Potential total; GWP-fossil = Global Warming Potential fossil fuels; GWP-biogenic = Global Warming Potential biogenic; GWP-luluc =
Global Warming Potential land use and land use change; ODP = Depletion potential of the stratospheric ozone layer; AP = Acidification potential, Accumulated
Exceedance; EP-freshwater = Eutrophication potential, fraction of nutrients reaching freshwater end compartment: EP-marine = Eutrophication potential, fraction of
nutrients reaching marine end compartment; EP-terrestrial = Eutrophication potential, Accumulated Exceedance; POCP = Formation potential of tropospheric ozone;
ADP-minerals&metals = Abiotic depletion potential for non-fossil resources; ADP-fossil = Abiotic depletion for fossil resources potential; WDP = Water (user)
deprivation potential, deprivation-weighted water consumption
"Reading example: 9,0 E-03 = 9,0*10-3 = 0,009"
*INA Indicator Not Assessed
1. The results of this environmental impact indicator shall be used with care as the uncertainties on these results are high or as there is limited experienced with the
indicator
Remarks to environmental impacts
7 / 12
Additional environmental impact indicators
Indicator Unit A1-A3 A4 C1 C2 C3 C4 D
PM Disease incidence 2,57E-03 4,26E-05 1,94E-06 2,66E-06 3,42E-06 2,60E-06 -3,96E-04
IRP2 kgBq U235 -eq 1,71E+03 4,60E+01 4,13E-01 2,88E+00 2,74E+00 2,01E+00 -8,27E+00
ETP-fw1 CTUe 2,85E+06 7,80E+03 5,26E+01 4,88E+02 4,34E+03 3,30E+03 -1,38E+06
HTP-c1 CTUh 1,87E-04 0,00E+00 0,00E+00 0,00E+00 1,50E-07 1,14E-06 -2,48E-05
HTP-nc1 CTUh 3,37E-03 8,52E-06 4,78E-08 5,33E-07 7,24E-06 7,61E-05 -1,45E-03
SQP1 dimensionless 1,83E+05 7,36E+03 1,22E+01 4,60E+02 2,51E+02 7,87E+02 -1,74E+04
PM = Particulate Matter emissions; IRP = Ionizing radiation – human health; ETP-fw = Eco toxicity – freshwater; HTP-c = Human toxicity – cancer effects; HTP-nc =
Human toxicity – non cancer effects; SQP = Potential Soil Quality Index (dimensionless)
"Reading example: 9,0 E-03 = 9,0*10-3 = 0,009"
*INA Indicator Not Assessed
1. The results of this environmental impact indicator shall be used with care as the uncertainties on these results are high or as there is limited experienced with the
indicator
2. This impact category deals mainly with the eventual impact of low dose ionizing radiation on human health of the nuclear fuel cycle. It does not consider effects due
to possible nuclear accidents, occupational exposure nor due to radioactive waste disposal in underground facilities. Potential ionizing radiation from the soil, from
radon and from some construction materials is also not measured by this indicator.
8 / 12
Resource use
Indicator Unit A1-A3 A4 C1 C2 C3 C4 D
PERE MJ 5,82E+04 1,51E+02 5,21E-01 9,42E+00 7,73E+01 4,89E+01 -4,24E+03
PERM MJ 6,48E+00 0,00E+00 0,00E+00 0,00E+00 -8,64E-02 0,00E+00 0,00E+00
PERT MJ 5,82E+04 1,51E+02 5,21E-01 9,42E+00 7,73E+01 4,89E+01 -4,24E+03
PENRE MJ 4,72E+05 1,05E+04 9,63E+01 6,58E+02 6,80E+02 5,00E+02 -1,92E+04
PENRM MJ 1,03E+04 0,00E+00 0,00E+00 0,00E+00 -1,03E+04 0,00E+00 0,00E+00
PENRT MJ 4,82E+05 1,05E+04 9,63E+01 6,58E+02 -9,58E+03 5,00E+02 -1,92E+04
SM kg 2,05E+03 0,00E+00 4,73E-02 0,00E+00 0,00E+00 6,37E-01 2,48E+02
RSF MJ 8,98E+02 5,39E+00 1,28E-02 3,37E-01 1,78E+00 6,73E-01 7,01E+01
NRSF MJ 4,31E+03 1,93E+01 1,89E-01 1,20E+00 -4,60E-01 6,68E+00 1,41E+03
FW m3 3,66E+02 1,13E+00 4,96E-03 7,04E-02 2,05E+00 1,56E+00 -2,50E+01
PERE = Use of renewable primary energy excluding renewable primary energy resources used as raw materials; PERM = Use of renewable primary energy resources used
as raw materials; PERT = Total use of renewable primary energy resources; PENRE = Use of non renewable primary energy excluding non-renewable primary energy
resources used as raw materials; PENRM = Use of non renewable primary energy resources used as raw materials; PENRT = Total use of non renewable primary energy
resources; SM = Use of secondary materials; RSF = Use of renewable secondary fuels; NRSF = Use of non-renewable secondary fuels; FW = Net use of fresh water
"Reading example: 9,0 E-03 = 9,0*10-3 = 0,009"
*INA Indicator Not Assessed
9 / 12
End of life - Waste
Indicator Unit A1-A3 A4 C1 C2 C3 C4 D
HWD kg 2,82E+02 5,43E-01 2,84E-03 3,39E-02 2,45E+00 4,52E+01 -1,60E+01
NHWD kg 1,26E+04 5,12E+02 1,14E-01 3,20E+01 3,77E+02 1,28E+03 -9,54E+02
RWD kg 1,47E+00 7,17E-02 6,69E-04 4,48E-03 1,40E-03 1,93E-03 -8,24E-03
HWD = Hazardous waste disposed; NHWD = Non-hazardous waste disposed; RWD = Radioactive waste disposed
"Reading example: 9,0 E-03 = 9,0*10-3 = 0,009"
*INA Indicator Not Assessed
End of life - Output flow
Indicator Unit A1-A3 A4 C1 C2 C3 C4 D
CRU kg 0,00E+00 0,00E+00 0,00E+00 0,00E+00 0,00E+00 0,00E+00 0,00E+00
MFR kg 3,74E+00 0,00E+00 4,64E-02 0,00E+00 3,47E+03 2,88E-02 -9,69E+00
MER kg 3,30E+00 0,00E+00 1,44E-04 0,00E+00 3,30E+01 4,64E-04 -1,28E+00
EEE MJ 3,45E-01 0,00E+00 4,94E-04 0,00E+00 4,20E+02 1,80E-02 -3,13E+00
EET MJ 5,22E+00 0,00E+00 7,47E-03 0,00E+00 6,35E+03 2,72E-01 -4,73E+01
CRU = Components for re-use; MFR = Materials for recycling; MER = Materials for energy recovery; EEE = Exported energy electrical; EET = Exported energy thermal
"Reading example: 9,0 E-03 = 9,0*10-3 = 0,009"
*INA Indicator Not Assessed
Biogenic Carbon Content
Indicator Unit At the factory gate
Biogenic carbon content in product kg C 0,00E+00
Biogenic carbon content in accompanying packaging kg C 0,00E+00
Note: 1 kg biogenic carbon is equivalent to 44/12 kg CO2
10 / 12
Additional requirements
Greenhouse gas emissions from the use of electricity in the manufacturing phase
National production mix from import, low voltage (production of transmission lines, in addition to direct emissions and losses in grid) of applied
electricity for the manufacturing process (A3).
Electricity mix Source Amount Unit
Electricity, Czech Republic (kWh) ecoinvent 3.6 942,91 g CO2-eq/kWh
Electricity, market mix (kWh) - Germany ecoinvent 3.6 585,93 g CO2-eq/kWh
Dangerous substances
The product contains dangerous substances, more than 0,1% by weight, given by the REACH Candidate List, see table:
Name CASNo Amount
Lead 7439-92-1 > 0.1 % w/w
2-methyl-1-(4-methylthiophenyl)-2-morpholinopropan-1-one 71868-10-5 > 0.1% w/w
Indoor environment
Additional Environmental Information
Additional environmental impact indicators required in NPCR Part A for construction products
Indicator Unit A1-A3 A4 C1 C2 C3 C4 D
GWPIOBC kg CO2 -eq 3,49E+04 6,97E+02 7,00E+00 4,35E+01 1,12E+03 8,69E+01 -2,40E+03
GWP-IOBC: Global warming potential calculated according to the principle of instantaneous oxidation. In order to increase the transparency of biogenic carbon​
contribution to climate impact, the indicator GWP-IOBC is required as it declares climate impacts calculated according to the principle of instantaneous oxidation.​
GWP-IOBC is also referred to as GWP-GHG in context to Swedish public procurement legislation.
11 / 12
Bibliography
ISO 14025:2010 Environmental labels and declarations - Type III environmental declarations - Principles and procedures.
ISO 14044:2006 Environmental management - Life cycle assessment - Requirements and guidelines.
EN 15804:2012+A2:2019 Environmental product declaration - Core rules for the product category of construction products.
ISO 21930:2017 Sustainability in buildings and civil engineering works - Core rules for environmental product declarations of construction
products.
ecoinvent v3, Allocation, cut-off by classification, Swiss Centre of Life Cycle Inventories.
Iversen et al., (2021) eEPD v2021.09 Background information for EPD generator tool system verification, LCA.no Report number: 07.21
Graafland and Iversen (2022) EPD generator for NPCR 030 Ventilation components, Background information for EPD generator application and
LCA data, LCA.no report number: 12.22
NPCR Part A: Construction products and services. Ver. 2.0. April 2021, EPD-Norge.
NPCR 030 Part B for Ventilation components, Ver. 1.0, 18.05.2021, EPD Norway.
EN ISO 9001:2015 - Quality management systems.
EN ISO 14001:2015 - Environmental management systems.
EN ISO 50001:2018 - Energy management systems.
Program operator and publisher Phone: +47 977 22 020
The Norwegian EPD Foundation e-mail: post@epd-norge.no
Post Box 5250 Majorstuen, 0303 Oslo, Norway web: www.epd-norge.no
Owner of the declaration: +49 2845 2020
Phone:
TROX Group productsustainability-
e-mail:
Heinrich-Trox-Platz 1, 47506 Neukirchen-Vluyn, de@troxgroup.com
web:
Germany https://www.trox.de/en
Author of the Life Cycle Assessment Phone: +47 916 50 916
LCA.no AS e-mail: post@lca.no
Dokka 6A, 1671 Kråkerøy, Norway web: www.lca.no
Developer of EPD generator Phone: +47 916 50 916
LCA.no AS e-mail: post@lca.no
Dokka 6A, 1671 Kråkerøy, Norway web: www.lca.no
ECO Platform web: www.eco-platform.org
ECO Portal web: ECO Portal
12 / 12
