ver1 2015
ENVIRONMENTALPRODU DECLARATION
CT
in accordance with ISO 14025, ISO 21930 and EN 15804
Owner of the declaration: Saint-Gobain Sweden AB, ISOVER
Program operator: The Norwegian EPD Foundation
Publisher: The Norwegian EPD Foundation
Declaration number: NEPD-2063-932-EN
Registration number: NEPD-2063-932-EN
ECO Platform reference number: -
Issue date: 06.03.2020
Valid to: 06.03.2025
ISOVER PLUS+ Skiva 32
Saint-Gobain Sweden AB, ISOVER
www.epd-norge.no
NEPD-2063-932-EN ISOVER PLUS+ Skiva 32
General information
Product Owner of the declaration
ISOVER PLUS+ Skiva 32 Saint-Gobain Sweden AB, ISOVER
Contact person: Daniel Odby
Program operator Phone:
+46 (0)42-842 52
e-mail:
daniel.odby@saint-gobain.com
The Norwegian EPD Foundation
Post Box 5250 Majorstuen, 0303
Manufacturer
Oslo Phone: +47 97722020
e-mail: post@epd-norge.no Saint-Gobain Sweden AB, ISOVER
www.epd-norge.no
Declaration number Place of production
NEPD-2063-932-EN Billesholm, Sweden
ECO Platform reference number Management system
SS-EN ISO 9001:2008
SS-EN ISO 14001:2004
This declaration is based on Product Category Rules Org. No
556241-2592
CEN Standard EN 15804 serve as core PCR
The Product Category Rules, NPCR 012:2018 Part B for
Thermal insulation products is used in addition to the core Issue date
PCR. 06.03.2020
Valid to
Statement of liability
06.03.2025
The owner of the declaration shall be liable for the
underlying information and evidence. EPD Norway
shall not be liable with respect to manufacturer
information, life cycle assessment data and evidences.
Year of study
Declared unit
2016
1 m² with a thermal resistance of 1.0 K m2 W-1
With a thickness of 32 mm.
Comparability
Functional unit
EPD of construction products may not be comparable if
1 m² with a thermal resistance of 1.0 K m2 W-1
they do not comply with EN15804 and seen in a
with a reference service life of 60 years.
building context.
Verification
The EPD has been worked out by
Independent verification of calculation data and other The EPD has been worked by the use of EPD
environmental information and test of the computer program tool, TEAM, version 5.2 by Saint-Gobain
was carried out by Martin Erlandsson in accordance with ISOVER TEAM by Michaël Medard and Sanna
ISO14025, 8.1.3 and 8.1.4 + EN 15804 Lindholm.
Externally Company-specific data has been verified by
Michaël Medard, Saint-Gobain Isover.
IVL Swedish Environmental Research Institute
(Independent verifier approved by EPD Norway)
Approved
NEPD-2063-932-EN ISOVER PLUS+ Skiva 32 1
Product description
Product description and description of use:
This EPD describes the potential environmental impacts of 1 m² of glass wool insulation, ISOVER
PLUS+ Skiva 32, with a thermal resistance equal to 1 K∙m²∙W-1.
The intended use of this EPD is to communicate scientifically based environmental information for
construction products, for the purpose of assessing the environmental performance of buildings.
ISOVER glass wool products are CE-marked according to the EN 13172 (2011) “Thermal Insulation
Products – Evaluation of Conformity” and EN 13162 (2012) “Thermal insulation Products for Buildings.
Factory made mineral wool (MW) Products. Specification”.
The production site of Saint-Gobain Sweden AB, ISOVER in Billesholm, uses a small amount of natural
and abundant raw materials (sand, soda, limestone, feldspar) and high share of recycled glass cullets
(more than 50% post-consumer recycled content of the glass). This material is converted by using fusion
and fiberizing techniques to produce glass wool. The products obtained come in the form of a "mineral
wool mat" consisting of a soft, airy structure.
On Earth, naturally, the best insulator is dry immobile air at 10°C: its thermal conductivity factor,
expressed in λ, is 0.025 W/(m∙K) (watts per meter Kelvin degree). The thermal conductivity of mineral
wool is close to immobile air as its lambda varies from 0.030 W/(m∙K) for the most efficient to 0.040 W/
(m∙K).
With its entangled structure, glass wool is a porous material that traps the air, making it one of the best
insulating materials. The porous and elastic structure of the wool also absorbs noise in the air and offers
acoustic correction inside premises. Glass wool mainly containing incombustible materials does not
react to fire.
Glass wool insulation is used in buildings as well as industrial facilities. It ensures a high level of
comfort, minimizes carbon dioxide (CO ) emissions by preventing heat losses through roofs, walls,
2
floors, pipes and boilers. It reduces noise and protects homes and industrial facilities against fire.
Correctly installed glass wool products and solutions do not require maintenance and last throughout
the lifetime of the building (which is set at 60 years as a default value in the model), or as long as
the insulated building component is a part of the building.
2
NEPD-2063-932-EN ISOVER PLUS+ Skiva 32
Technical data/physical characteristics:
The thermal resistance of the product: 1.00 K∙m2∙W-1
The thermal conductivity of the product: 0.032 W/ (m∙K)
Reaction to fire: Euroclass A1
Description of the main product components and or materials:
Main components
Glass wool 90-95 % (REACH registration number 01-2119472313-44-0041)
Binder 0-10%
PARAMETER VALUE
Quantity of mineral wool 896 g
Thickness of mineral wool 32 mm
Surfacing No facing
Polyethylene 26.9 g
Packaging for the transportation and distribution
Wood pallet 115 g
Product used for the Installation: None
LCA calculation information
Providing a thermal insulation on 1 m² with a thermal
FUNCTIONALUNIT
resistance of equals 1 K.m2.W-1.
SYSTEM BOUNDARIES Cradle to Gate with options: A1-3, A4-5, B1- 7, C1-4
REFERENCE SERVICELIFE(RSL) 60 years
CUT-OFFRULES See detailed explanation page 9
ALLOCATIONS See detailed explanation page 9
ELECTRICITY USED FOR
Sweden electricity mix from IEA
THE MANUFACTORING
(reference year 2014)
PROCESS
GEOGRAPHICAL
COVERAGE AND TIME
Sweden 2016
PERIOD
GREENHOUSEGAS EMISSION
FROMELECTRICITY
Which equals 0.0056 kg CO2 eq /MJ
3
NEPD-2063-932-EN ISOVER PLUS+ Skiva 32
Flow diagram of the Life Cycle
4
NEPD-2063-932-EN ISOVER PLUS+ Skiva 32
System boundaries (X=included, MND=module not declared)
Beyond the
Construction
Product stage Use stage End of life stage system
installation stage
boundaries
5
slairetam
waR
tropsnarT
gnirutcafunaM
tropsnarT
noitallatsni
noitcurtsnoC
egats esU
ecnanetniaM
riapeR
tnemecalpeR tnemhsibrufeR
esu
ygrene
lanoitarepO
esu
retaw
lanoitarepO
noitcurtsnoc-eD
noitilomed tropsnarT
gnissecorp
etsaW
lasopsiD
-yrevoceR-esueR laitnetop-gnilcyceR
A1 A2 A3 A4 A5 B1 B2 B3 B4 B5 B6 B7 C1 C2 C3 C4 D
X X X X X X X X X X X X X X X X MND
Product stage, A1-A3
Description of the stage:
The product stage of the mineral wool products is subdivided into 3 modules A1, A2 and A3 respectively
“Raw material supply”, “transport” and “manufacturing”.
The aggregation of the modules A1, A2 and A3 is a possibility considered by the EN 15 804 standard. This
rule is applied in this EPD.
A1, Raw material supply
This module takes into account the extraction and processing of all raw materials and energy which occur
upstream to the studied manufacturing process.
Specifically, the raw material supply covers production of binder components and sourcing (quarry) of raw
materials for fiber production, e.g. sand and borax for glass wool. Besides these raw materials, recycled
material/glass cullet is also used as input.
About cullet: The main raw material for the production of glass insulation material is cullets or/and sand. Only
specific cleaning activities and transport is included for the cullets – and thus not the impacts from the full life
cycle of glass. The reason is that cullets are considered a waste product and not initially produced for the
purpose of glass wool insulation production. The only activities included are:
• Magnetic separation of metallic piece
• Separation of other piece-crushing of glass (<20 mm)
• Separation of bottle cap crushing (<2 mm) sieving
• Transport
A2, transport to the manufacturer
The raw materials are transported to the manufacturing site. In our case, the modeling include: road and boat
transportations (specific values) of each raw material.
A3, manufacturing
This module covers glass wool fabrication, including melting and fiberization (see process flow diagram).In
addition, the production of packaging material is taking into account at this stage.
NEPD-2063-932-EN ISOVER PLUS+ Skiva 32
Manufacturing process flow diagram
Construction process stage, A4-A5
Description of the stage:
The construction process is divided into 2 modules: A4, transport to the building site and A5, installation in
the building.
Description of scenarios and additional technical information:
A4, Transport to the building site:
- This module includes transport from the production gate to the building site. (Representative as
average for the Swedish market).
- Transport is calculated on the basis of a scenario with the parameters described in the following
table.
PARAMETER VALUE
Fuel type and consumption of vehicle or vehicle
Average truck trailer with a 24t payload, diesel
type used for transport e.g. long distance truck,
consumption 38 liters for 100 km
boat, etc.
Distance 500 km
95 % of the capacity in volume
Capacity utilisation (including empty returns)
50 % of empty returns
Bulk density of transported products 50-100 kg/m3
Volume capacity utilisation factor 1 (by default)
A5, Installation in the building: This module includes
6
NEPD-2063-932-EN ISOVER PLUS+ Skiva 32
- Wastage of products: see following table 5 %. These losses are landfilled (landfill model for glass
see chapter End of life),
- Additional production processes to compensate for the loss
- Processing of packaging wastes: they are 100 % collected and modeled as recovered matter.
PARAMETER VALUE
Wastage of materials on the building site before
waste processing, generated by the product’s 5 %
installation (specified by type)
Output materials (specified by type) as results of
Packaging wastes are 100 % collected and modeled
waste processing at the building site e.g. of
as recovered matter
collection for recycling, for energy recovering,
disposal
Glass wool losses are landfilled
(specified by route)
Use stage (excluding potential savings), B1-B7
Description of the stage: The use stage is divided into the following modules:
- B1: Use
- B2:Maintenance
- B3: Repair
- B4: Replacement
- B5: Refurbishment
- B6: Operational energyuse
- B7: Operational water use
Description of scenarios and additional technical information:
Once installation is complete, no actions or technical operations are required during the use stages
until the end of life stage. Therefore glass wool insulation products have no impact (excluding
potential energy savings) on this stage.
7
NEPD-2063-932-EN ISOVER PLUS+ Skiva 32
End-of-life stage C1-C4
Description of the stage:
The stage includes the different modules of end-of-life detailed below.
C1,de-construction,demolition
The de-construction and/or dismantling of insulation products take part of the demolition of the entire
building and is assumed to be made manually. In our case, the environmental impact is assumed to be
very small and can be neglected.
C2, transport to waste processing
Transport is included and calculated on the basis of a scenario with the parameters described in the
End-of-life table.
C3, waste processing for reuse, recovery and/or recycling;
Today the product is considered to be landfilled without reuse, recovery or
recycling.
C4, disposal;
The glass wool is assumed to be 100% landfilled.
Description of scenarios and additional technical information: See below
End-of-life:
PARAMETER VALUE/DESCRIPTION
The entire insulation product (wool and surfacing) is
Collection process specified by type
collected with mixed construction waste
Recovery system specified by type No re-use, recycling or energy recovery
The entire insulation product (wool and surfacing) is
Disposal specified by type
landfilled
Average truck trailer with a 24t payload, diesel
consumption 38 liters for 100 km
Assumptions for scenario development (e.g.
transportation)
25 km (default distance from the building site to
landfill).
Reuse/recovery/recycling potential, D
Module D is not included in the EPD.
8
NEPD-2063-932-EN ISOVER PLUS+ Skiva 32
LCA results
LCA model, aggregation of data and potential environmental impact are calculated from the TEAM™
software 5.2. and CML impact method has been used, together with DEAM (2017) and Ecoinvent V3.3
(2016) databases to obtain the inventory of generic data. Biogenic carbon is not reported in the context
of GWP.
Raw materials and energy consumption, as well as transport distances have been taken directly from
the manufacturing plant of Saint-Gobain Sweden A, ISOVER in Billesholm (Production data according
2016).
Resume of the LCA results detailed on the following tables.
Cut-off criteria
The cut-off criterion used in Saint-Gobain EPD will be the mass criterion with the following details:
- Taking into account all input and output flows in a unit process i.e. taking into account the
value of all flows in the unit process and the corresponding LCI whenever available
- No simplification of the LCI by additional exclusions of material flows
Data collected at the manufacturing site was used. The inventory process in this LCA includes all data
related to raw material, packaging material and consumable items, and the associated transport to the
manufacturing site. Process energy and water use, direct production waste and emissions to air and
water are included. Scenarios have been developed to account for downstream processes such as
demolition and waste treatment in accordance with the requirements of EN 15804:2012+A1:2013
All inputs and outputs to the manufacturing plants have been included and made transparent. All
assumptions regarding the materials and water balances have also been included.
All hazardous and toxic materials and substances are considered in the inventory even though they are
below the cut off criteria
There are excluded processes in the inventory:
- Flows related to human activities such as employee transport and administration activity.
Allocation
Allocation criteria are based on mass.
The allocation of all the air emissions, wastes and energy usage are based on mass (kg). The reason
we can use a mass basis is because we use the exact same manufacturing process shown for every
product. We only produce glass mineral wool in the Billesholm site using the same process and therefore
all the factors can be allocated by a mass basis. The amount of binder varies for different products and
is accounted for as well as if different surface layers are used.
A mass balance was conducted for the 2016 production year to ensure that we haven’t excluded any
materials, emissions and hence potential environmental impacts. Regarding the mass balance, all the
raw materials and corresponding production goods and wastes generated were taken into account.
9
NEPD-2063-932-EN ISOVER PLUS+ Skiva 32
Influence of particular thicknesses
All the results in the table of this EPD refer to an ISOVER PLUS+ Skiva 32 with a 32 mm of thickness
for a functional unit of 1 m² with a thermal resistance equals to 1 K∙m²∙W-1.
Other Environmental impact indictor result based on the same requirements can be provided for other
R-values (other thicknesses) for ISOVER PLUS+ Skiva 32 after request.
10
NEPD-2063-932-EN ISOVER PLUS+ Skiva 32
ENVIRONMENTAL IMPACTS
Product Construction
Use stage End-of-life stage
stage process stage
Parameters
11
3A
/
2A
/
1A
tropsnarT
4A
noitallatsnI
5A
esU
1B
ecnanetniaM
2B
riapeR
3B
4B
tnemecalpeR
5B
tnemhsibrufeR lanoitarepO
6B
esu
ygrene
lanoitarepO
7B
esu
retaw 1C
/ noitcurtsnoceD noitilomed tropsnarT
2C
etsaW
3C
gnissecorp lasopsiD
4C
,yrevocer
,esueR
D
gnilcycer
7.1E-01 8.1E-02 4.0E-02 0 0 0 0 0 0 0 0 5.8E-03 0 4.8E-03 MND
Global Warming Potential
(GWP) - kg CO2 equiv/FU
The global warming potential of a gas refers to the total contribution to global warming resulting from the emission
of one unit of that gas relative to one unit of the reference gas, carbon dioxide, which is assigned a value of 1.
4.7E-08 5.9E-08 5.5E-09 0 0 0 0 0 0 0 0 4.2E-09 0 1.6E-09 MND
Ozone Depletion (ODP)
kg CFC 11 equiv/FU Destruction of the stratospheric ozone layer which shields the earth from ultraviolet radiation harmful to life.
This destruction of ozone is caused by the breakdown of certain chlorine and/or bromine containing compounds (chlorofluorocarbons or halons),
which break down when they reach the stratosphere and then catalytically destroy ozone molecules.
5.6E-03 3.7E-04 3.0E-04 0 0 0 0 0 0 0 0 2.7E-05 0 3.6E-05 MND
Acidification potential (AP)
kg SO2 equiv/FU
Acid depositions have negative impacts on natural ecosystems and the man-made environment incl, buildings.
The main sources for emissions of acidifying substances are agriculture and fossil fuel combustion used for electricity production, heating and transport.
Eutrophication potential (EP) 6.9E-04 8.8E-05 3.9E-05 0 0 0 0 0 0 0 0 6.3E-06 0 6.5E-06 MND
kg (PO4)3- equiv/FU
Excessive enrichment of waters and continental surfaces with nutrients, and the associated adverse biological effects.
Photochemical ozone 6.3E-04 5.8E-05 3.5E-05 0 0 0 0 0 0 0 0 4.2E-06 0 1.0E-05 MND
creation (POPC)
kg Ethene equiv/FU Chemical reactions brought about by the light energy of the sun.
The reaction of nitrogen oxides with hydrocarbons in the presence of sunlight to form ozone is an example of a photochemical reaction.
Abiotic depletion potential for
non-fossil ressources (ADP- 8.4E-07 2.2E-11 4.2E-08 0 0 0 0 0 0 0 0 1.6E-12 0 4.2E-09 MND
elements) - kg Sb equiv/FU
Abiotic depletion potential for
1.4E+01 1.0E+00 7.6E-01 0 0 0 0 0 0 0 0 7.5E-02 0 1.4E-01 MND
fossil ressources (ADP-fossil
fuels) - MJ/FU
Consumption of non-renewable resources, thereby lowering their availability for future generations.
NEPD-2063-932-EN ISOVER PLUS+ Skiva 32
RESOURCE USE
Product Construction
Use stage End-of-life stage
stage process stage
Parameters
12
3A
/
2A
/
1A
tropsnarT
4A
noitallatsnI
5A
esU
1B
ecnanetniaM
2B
riapeR
3B
4B
tnemecalpeR
5B
tnemhsibrufeR lanoitarepO
6B
esu
ygrene
lanoitarepO
7B
esu
retaw 1C
/ noitcurtsnoceD noitilomed tropsnarT
2C
etsaW
3C
gnissecorp lasopsiD
4C
,yrevocer
,esueR
D
gnilcycer
Use of renewable primary
energy excluding renewable
2.1E+00 5.1E-04 2.1E-01 0 0 0 0 0 0 0 0 3.6E-05 0 3.5E-03 MND
primary energy resources used
as raw materials - MJ/FU
Use of renewable primary
energy used as raw materials 2.1E+00 0 0 0 0 0 0 0 0 0 0 0 0 0 MND
MJ/FU
Total use of renewable primary energy
resources (primary energy and
4.2E+00 5.1E-04 2.1E-01 0 0 0 0 0 0 0 0 3.6E-05 0 3.5E-03 MND
primary energy resources used as raw
materials) MJ/FU
Use of non-renewable primary
energy excluding non-renewable
2.0E+01 1.0E+00 1.1E+00 0 0 0 0 0 0 0 0 7.5E-02 0 1.4E-01 MND
primary energy resources used
as raw materials - MJ/FU
Use of non-renewable primary
energy used as raw materials 0 0 0 0 0 0 0 0 0 0 0 0 0 0 MND
MJ/FU
Total use of non-renewable primary
energy resources (primary energy and
2.0E+01 1.0E+00 1.1E+00 0 0 0 0 0 0 0 0 7.5E-02 0 1.4E-01 MND
primary energy resources used as raw
materials) - MJ/FU
Use of secondary material
4.8E-01 0 2.4E-02 0 0 0 0 0 0 0 0 0 0 0 MND
kg/FU
Use of renewable secondary
0 0 0 0 0 0 0 0 0 0 0 0 0 0 MND
fuels- MJ/FU
Use of non-renewable
0 0 0 0 0 0 0 0 0 0 0 0 0 0 MND
secondary fuels - MJ/FU
1.44E- 9.96E- 7.32E- 7.14E- 1.49E-
Use of net fresh water - m3/FU 0.0 0.0 0.0 0.0 0.0 0.0 0.0 0.0 0.0 MND
02 05 04 06 04
NEPD-2063-932-EN ISOVER PLUS+ Skiva 32
WASTE CATEGORIES
Product Construction
Use stage End-of-life stage
stage process stage
Parameters
13
3A
/
2A
/
1A
tropsnarT
4A
noitallatsnI
5A
esU
1B
ecnanetniaM
2B
riapeR
3B
4B
tnemecalpeR
5B
tnemhsibrufeR lanoitarepO
6B
esu
ygrene
lanoitarepO
7B
esu
retaw 1C
/ noitcurtsnoceD noitilomed tropsnarT
2C
etsaW
3C
gnissecorp lasopsiD
4C
,yrevocer
,esueR
D
gnilcycer
Hazardous waste disposed
3.7E-02 3.2E-05 1.9E-03 0 0 0 0 0 0 0 0 2.3E-06 0 7.0E-05 MND
kg/FU
Non-hazardous waste disposed
3.0E-01 8.6E-05 6.0E-02 0 0 0 0 0 0 0 0 6.2E-06 0 9.0E-01 MND
kg/FU
Radioactive waste disposed
6.1E-05 1.7E-05 4.0E-06 0 0 0 0 0 0 0 0 1.2E-06 0 9.1E-07 MND
kg/FU
NEPD-2063-932-EN ISOVER PLUS+ Skiva 32
OUTPUT FLOWS
Product Construction
Use stage End-of-life stage
stage process stage
Parameters
14
3A
/
2A
/
1A
tropsnarT
4A
noitallatsnI
5A
esU
1B
ecnanetniaM
2B
riapeR
3B
4B
tnemecalpeR
5B
tnemhsibrufeR lanoitarepO
6B
esu
ygrene
lanoitarepO
7B
esu
retaw 1C
/ noitcurtsnoceD noitilomed tropsnarT
2C
etsaW
3C
gnissecorp lasopsiD
4C
,yrevocer
,esueR
D
gnilcycer
Components for re-use
0 0 0 0 0 0 0 0 0 0 0 0 0 0 MND
kg/FU
Materials for recycling
2.6E-01 0 1.6E-01 0 0 0 0 0 0 0 0 0 0 0 MND
kg/FU
Materials for energy recovery
0 0 0 0 0 0 0 0 0 0 0 0 0 0 MND
kg/FU
Exported energy
6.9E-07 0 3.5E-08 0 0 0 0 0 0 0 0 0 0 0 MND
MJ/FU
NEPD-2063-932-EN ISOVER PLUS+ Skiva 32
LCA interpretation
Product Transport Installation Use End-of-life
(A1-A3) (A4) (A5) (B) (C) Total Recycling
Environmental Positive benefits
impacts of the of recycling
product (D)
Global warming 0.80 0.71
0.60
0.84
0.40
0.20 0.08 0.04 0.00 0.01 0.00
0.00
Non-renewable resources 15.00 13.92
consumption [1]
10.00 15.93
5.00
1.04 0.76 0.00 0.21 0.00
0.00
Energy consumption [2] 30.00 24.52
20.00 27.08
10.00
1.05 1.29 0.00 0.21 0.00
0.00
Water consumption [3] 0.02
0.01
0.02
0.015
0.01
0.01 0.00 0.00 0.00 0.00 0.00
0.00
Waste production [4] 1.00 0.90
1.30
0.50 0.34
0.00 0.06 0.00 0.00
0.00
[1] This indicator corresponds to the abiotic depletion potential of fossil resources.
[2] This indicator corresponds to the total use of primary energy.
[3] This indicator corresponds to the use of net fresh water.
[4] This indicator corresponds to the sum of hazardous, non-hazardous and radioactive waste disposed.
Additional Norwegian requirements
Greenhous gas emission from the use of electricity in the manufacturing phase
Electricity use in production is based on consumption figures for 2014 in Sweden according to IEA 2016
figures.
Emission data is taken from the module in TEAM/DEAM database “_401 Electricity (Sweden, 2014)”.
Indoor environment
The EPD does not give any information on release of regulated dangerous substances to indoor air because
the national regulation in Sweden does not require any verification and declaration of release of regulated
dangerous substances today.
Dangerous substances
The product contains no substances given from the REACH Candidate list (of 07.07.2017)
(REACH registration number 01-2119472313-44-0041)
UF/viuqe2OC
gk
UF/JM
UF/JM
UF/3m
UF/gk
kg CO2equiv/FU
MJ/FU
MJ/FU
m3/FU
kg/FU
Data source Amount Unit
TEAM/DEAM_401 Electricity (Sweden, 2014)”. 20,29 gram CO2-eqv/kWh
NEPD-2063-932-EN ISOVER PLUS+ Skiva 32
Bibliography
- Product-Category Rules, EPD Norway. NPCR 012:2018 Part B for Thermal
insulation products is used in addition to the core PCR (2018).
- Environmental labels and declarations - Type III environmental declarations -
Principles and procedures (ISO 14025:2006)
- Environmental management - Life cycle assessment –
Requirements and guidelines (ISO 14044:2006)
- Sustainability of construction works - Environmental product declaration - Core rules
for the product category of construction products (EN 15804:2012)
- Sustainability in building construction - Environmental declaration of building products (ISO
21930:2007)
- LCA report Saint -Gobain ISOVER May 2017 (revised December 2019)
- Ecoinvent database V3.3 (2016) information about validation, calculation, and update
are available via the various reports:
o ecoinvent 2.2 translated reports_06_Energy Systems.zip 23 MB 08.08.2016
o ecoinvent 3 report_Crop Production.zip 2.2 MB 08.08.2016
o ecoinvent 3 report_Refrigerated Transport.pdf 845.2 KB 08.08.2016
o ecoinvent 3 report_selected chapters_Energy.zip 293 KB 08.08.2016
o ecoinvent 3 report_Transport Default Model_Global.pdf 464.9 KB 08.08.2016
o ecoinvent 3 report_Transport Default Model_Switzerland.zip 636.5 KB 08.08.2016
o ecoinvent 3.3 open access datasets_PDF documentation.zip
All these report are available at: https://v33.ecoquery.ecoinvent.org/File/Reports
- Ecobilan DEAM database, information about validation, calculation, and update
are available via the report:
o DEAM™ User's Manual Version 2017 DEAMSTK 5.2.4
This user manual is only available with the license of the tool.
- SS-EN 13172:2012 Thermal Insulation Products – Evaluation of conformity
- SS-EN 13162:2012 Thermal insulation products for buildings – Factory made
mineral wool (MW) products – Specification
Program operator and Publisher Phone: +47 97722020
The Norwegian EPD Foundation
Post Box 5250 Majorstuen, 0303 Oslo e-mail: post@epd-norge.no
Norway web www.epd-norge.no
Owner of the declaration Phone: +46 (0)42-842 52
Saint-Gobain Sweden AB, ISOVER e-mail: daniel,odby@saint-
gobain,com
web www.isover.se
Author of the Life Cycle Assessment Phone: +33 1 40 99 24 04
Michael Medard e-mail: Michael.medard@saint-
Saint-Gobain ISOVER gobain.com
France web <wxwxwxx.i>so ver.com
16
NEPD-2063-932-EN ISOVER PLUS+ Skiva 32
