Environmental product declaration
in accordance with ISO 14025 and EN 15804+A2
LAPP ÖLFLEX® CLASSIC 135 CH 7G0,75 Elnr 1071204
Owner of the declaration: Program operator:
Lapp Norway AS The Norwegian EPD Foundation
Product: Declaration number:
LAPP ÖLFLEX® CLASSIC 135 CH 7G0,75 Elnr 1071204 NEPD-8813-8463
Declared unit: Registration number:
1 m NEPD-8813-8463
This declaration is based on Product Category Rules: Issue date:
CEN Standard EN 15804:2012+A2:2019 serves as core 23.01.2025
PCR
Valid to:
The Norwegian EPD Foundation NPCR 027:2020 Part B for Electrical cables and wires
23.01.2030
EPD software:
LCAno EPD generator ID: 750128
1 / 12
General information
Product Owner of the declaration:
LAPP ÖLFLEX® CLASSIC 135 CH 7G0,75 Elnr 1071204 Lapp Norway AS
Contact person: Petter Dahl
Phone: 91597046
e-mail: petter.dahl@lapp.com
Program operator: Manufacturer:
The Norwegian EPD Foundation Lapp Norway AS
Post Box 5250 Majorstuen, 0303 Oslo, Norway Eikringen 11
Phone: +47 977 22 020 3036 Drammen, Norway
web: www.epd-norge.no
Declaration number: Place of production:
Cableries Lapp S.a.r.l.
NEPD-8813-8463 Technopole Sud Forbach
F - 57600 FORBACH, France
This declaration is based on Product Category Rules: Management system:
CEN Standard EN 15804:2012+A2:2019 serves as core PCR ISO 14001, ISO 9001
NPCR 027:2020 Part B for Electrical cables and wires
Statement of liability: Organisation no:
The owner of the declaration shall be liable for the underlying 919 398 876
information and evidence. EPD Norway shall not be liable with respect
to manufacturer information, life cycle assessment data and
evidences.​
Declared unit: Issue date:
1 m LAPP ÖLFLEX® CLASSIC 135 CH 7G0,75 Elnr 1071204 23.01.2025
Declared unit with option: Valid to:
A1,A2,A3,A4,A5,C1,C2,C3,C4,D 23.01.2030
Year of study:
2023
Functional unit: Comparability:
1 meter of ÖLFLEX® CLASSIC 135 CH7G0,75 mm2 from cradle-to- EPD of construction products may not be comparable if they not
grave. comply with EN 15804 and seen in a building context.
General information on verification of EPD from EPD tools: Development and verification of EPD:
Independent verification of data, other environmental information The declaration is created using EPD tool lca.tools ver EPD2022.03,
and the declaration according to ISO 14025:2010, § 8.1.3 and § 8.1.4. developed by LCA.no. The EPD tool is integrated in the company's
Verification of each EPD is made according to EPD-Norway’s management system, and has been approved by EPD Norway.
guidelines for verification and approval requiring that tools are i) Approval number: NEPDT133
integrated into the company's environmental management system, ii)
the procedures for use of the EPD tool are approved by EPD-Norway, Developer of EPD: Julie Olsson
and iii) the process is reviewed annually by an independent third
Reviewer of company-specific input data and EPD:​ Lars Nilsen
party verifier. See Appendix G of EPD-Norway's General Programme
Instructions for further information on EPD tools
Verification of EPD tool: Approved:
Independent third party verification of the EPD tool, background data
and test-EPD in accordance with EPDNorway's procedures and
guidelines for verification and approval of EPD tools. Approval
number: NEPDT32.
Third party verifier:
Vito D’Incognito, Take Care International
(no signature required)
2 / 12
Product
Product description:
ÖLFLEX CLASSIC 135 CH are screened halogen free, highly flame retardant control cables designed for the European and North American
market, for occasional flexible use and fixed installation subject to normal mechanical load conditions.
They are also suitable for use in dry or damp areas. Considering the temperature range, a temporary outdoor use is possible. They are
suitable for occasional, non-automated movements. The maximum tensile load is 15 N/mm² of conductor cross-section during installation
and operation. Compulsory guidance is not permitted.
The screening braid protects against interference from electrical fields.
Application range: Public buildings, airports, railway stations, plant engineering and construction, air conditioning systems and particularly
where human and animal life as well as valuable property are exposed to high risk of fire hazards. In the event of a fire minimal toxic and no
corrosive gases occur.
USE according to UL: FRPE sheathed cable for internal wiring of appliances
Product specification
Design acc. to UL AWM Style 10701 and 21217 and UL 758,
and based on EN 50525-3-11
Certification UL AWM Style 21217* (File No. E63634), UL 758
DNV Certificate No. TAE00002RK
VDE certified: Supply cable with improved characteristics in the case of fire
EN 13501-6 and EN 50575
Classification of fire behaviour
(article/dimension range see www.lappkabel.com/cpr)
*Style change: UL Style 21089 replaced by Style 21217 (approx. February 2018)
Conductor fine wire strands of bare copper, acc. to IEC 60228 resp. EN 60228, Class 5
Insulation halogen free compound TI6,
acc. to EN 50363-7, with increased requirements
Core identification code acc. to VDE 0293-1, with or without GN/YE ground conductor
black cores with white numbers acc. to DIN EN 50334
Stranding cores are stranded in layers
Wrapping plastic foil
Screen braid of tinned copper, coverage = 85% (nominal value)
Outer sheath halogen free compound TM7 acc. to EN 50363-8
Colour: Silver grey, similar RAL 7001
Materials kg %
HFFR Polyolefin 0,04 31,01
Metal - Copper 0,09 68,99
Total 0,13 100,00
Packaging kg %
Packaging - Wood 0,01 100,00
Total incl. packaging 0,13 100,00
Technical data:
3 / 12
Electrical properties at 20 °C
Transfer impedance at 30 MHZ max. 250 O/km acc. to EN 50395
Nominal voltage EN U0/U: 300/500 V
UL: 600 V
Test voltage core / core: 4000 V AC
core / screen: 2000 V AC
Mechanical and thermal properties
Minimum bending radius occasional flexing: 20 x outer diameter
fixed installation: 6 x outer diameter
Temperature range occasional flexing (EN): -25°C up to +70°C max. conductor temp.
occasional flexing (UL): up to +75°C max. conductor temp.
fixed installation (EN): -40°C up to +80°C max. conductor temp.
fixed installation (UL): up to +75°C max. conductor temp.
Flammability flame retardant acc. to IEC 60332-1-2 resp. EN 60332-1-2
UL: Horizontal flame test acc. to UL 1581 §1090
no flame-propagation
acc. to IEC 60332-3-22 resp. EN 60332-3-22
acc. to IEC 60332-3-24 resp. EN 60332-3-24 or
acc. to IEC 60332-3-25 resp. EN 60332-3-25
Halogen free acc. to IEC 60754-1 resp. EN 60754-1
Corrosivity of gases acc. to IEC 60754-2 resp. EN 60754-2
Smoke density acc. to IEC 61034-2 resp. EN 61034-2
Toxicity acc. to EN 50306-1 (= 6)
UV resistance acc. to EN 50620
acc. to EN ISO 4892-2-2013, method A (change of colour allowed)
Ozone resistance acc. to EN 50396 resp., method B
.
Tests acc. to IEC 60811 resp. EN 60811, EN 50395, EN 50396, UL 1581
General requirements These cables are conform to the EU-Directive 2014/35/EU (Low Voltage Directive).
A part of these cables (see www.lappkabel.com/cpr) are classified
in accordance with the EU-Regulation no. 305/2011 (CPR).
Environmental information These cables meet the substance-specific requirements of the EU Directive 2011/65/EU (RoHS).
Market:
Norway
Reference service life, product
Expected lifetime 40 years, provided proper installation, load and ambient temperature.
Reference service life, building or construction works
40 years
LCA: Calculation rules
Declared unit:
1 m LAPP ÖLFLEX® CLASSIC 135 CH 7G0,75 Elnr 1071204
Cut-off criteria:
All major raw materials and all the essential energy is included. The production processes for raw materials and energy flows with very small
amounts (less than 1%) are not included. These cut-off criteria do not apply for hazardous materials and substances.
Allocation:
The allocation is made in accordance with the provisions of EN 15804. Incoming energy and water and waste production in-house is allocated
equally among all products through mass allocation. Effects of primary production of recycled materials is allocated to the main product in which
the material was used. The recycling process and transportation of the material is allocated to this analysis.
Data quality:
Specific data for the product composition are provided by the manufacturer. The data represent the production of the declared product and were
collected for EPD development in the year of study. Background data is based on EPDs according to EN 15804 and different LCA databases. The
data quality of the raw materials in A1 is presented in the table below.
Materials Source Data quality Year
HFFR Polyolefin ecoinvent 3.6 Database 2019
Metal - Copper ecoinvent 3.6 Database 2019
Packaging - Wood ecoinvent 3.6 Database 2019
4 / 12
System boundaries (X=included, MND=module not declared, MNR=module not relevant)
Construction Beyond the system
Product stage Use stage End of life stage
installation stage boundaries
A1 A2 A3 A4 A5 B1 B2 B3 B4 B5 B6 B7 C1 C2 C3 C4 D
X X X X X MND MND MND MND MND MND MND X X X X X
System boundary:
1m LAPP ÖLFLEX® CLASSIC 135 CH 7G0,75 Elnr 1071204
The flowchart below illustrates the system boundaries of the analysis:
Additional technical information:
The article 1071204 ÖLFLEX CLASSIC 135 CH 7G0,75 represents the product with the highest expenditure of raw materials and energy
consumption during manufacturing of all the following products from the same product family:
Elnumber Article no:
1070985 1123200 ÖLFLEX® CLASSIC 135 CH 2X0,5
1070986 1123201 ÖLFLEX® CLASSIC 135 CH 3G0,5
1070987 1123202 ÖLFLEX® CLASSIC 135 CH 3X0,5
1070988 1123203 ÖLFLEX® CLASSIC 135 CH 4G0,5
1070989 1123204 ÖLFLEX® CLASSIC 135 CH 4X0,5
1070990 1123205 ÖLFLEX® CLASSIC 135 CH 5G0,5
1070991 1123206 ÖLFLEX® CLASSIC 135 CH 5X0,5
1070992 1123208 ÖLFLEX® CLASSIC 135 CH 7G0,5
1070993 1123209 ÖLFLEX® CLASSIC 135 CH 7X0,5
1070997 1123232 ÖLFLEX® CLASSIC 135 CH 2X0,75
1070998 1123233 ÖLFLEX® CLASSIC 135 CH 3G0,75
1070999 1123234 ÖLFLEX® CLASSIC 135 CH 3X0,75
1071200 1123235 ÖLFLEX® CLASSIC 135 CH4G0,75
1071201 1123236 ÖLFLEX® CLASSIC 135 CH4X0,75
1071202 1123237 ÖLFLEX® CLASSIC 135 CH5G0,75
1071203 1123238 ÖLFLEX® CLASSIC 135 CH5X0,75
1071204 1123241 ÖLFLEX® CLASSIC 135 CH7G0,75
1071205 1123242 ÖLFLEX® CLASSIC 135 CH7X0,75
1071210 1123266 ÖLFLEX® CLASSIC 135 CH 2X1
1071211 1123267 ÖLFLEX® CLASSIC 135 CH 3G1
1071212 1123268 ÖLFLEX® CLASSIC 135 CH 3X1
1071213 1123269 ÖLFLEX® CLASSIC 135 CH 4G1
1071214 1123270 ÖLFLEX® CLASSIC 135 CH 4X1
1071215 1123271 ÖLFLEX® CLASSIC 135 CH 5G1
1071216 1123272 ÖLFLEX® CLASSIC 135 CH 5X1
1071224 1123306 ÖLFLEX® CLASSIC 135 CH 2X1,5
1071225 1123307 ÖLFLEX® CLASSIC 135 CH 3G1,5
1071226 1123308 ÖLFLEX® CLASSIC 135 CH 3X1,5
This EPD is only valid for the declared product.
waR slairetam tropsnarT gnirutcafunaM tropsnarT ylbmessA e​sU ecnanetniaM riapeR tnemecalpeR tnemhsibrufeR lanoitarepO ygrene esu lanoitarepO esu retaw -eD noitcurtsnoc noitilomed tropsnarT etsaW gnissecorp lasopsiD -yrevoceR-esueR laitnetop-gnilcyceR
5 / 12
LCA: Scenarios and additional technical information
The following information describe the scenarios in the different modules of the EPD.
Module A4 = In A4, a transport distance from the production site to LAPP Norways warehouse in Drammen was included. A distance of 300 km
was also added as additional transport to market.
Modules A5 = 5 % product losses during installation are estimated by the company. No energy use has been quantified since installation in
buildings is often done by manual labour. Use of portable electrical devices (e.g., drill) usually have low energy requirements falling under the cut​off
criterion of 1%. Cable drums are reused and also assumed under the cut-off criterion of 1%.
Module C1 = de-construction in buildings is often done by manual labour. Use of portable electrical devices (e.g., drill) usually have low energy
requirements falling under the cut-off criterion of 1%.
Module C2 = 85 km is added as an average distance to the waste facility
Modules C3 and C4 = Waste treatment of the product follows the default values provided in EN 50693, Product Category Rules for life cycle
assessments of electronic and electrical products and systems, table G.4. This table specified how different types of raw materials used in A1 will
likely be treated during the end-of-life of the product. Waste treatments in C3 include material recycling and incineration with and without energy
recovery and fly ash extraction. Disposal in C4 consist of landfilling of different waste fractions and of ashes.
Module D = The recyclability of metals and plastics allows the producers a credit for the net scrap that is produced at the end of a product’s life.
The benefits from recycling of net scrap are described in formula from EN 15804:2012+A2:2019. Substitution of heat and electricity generated by
the incineration with energy recovery of plastic insulation and other parts is also calculated in module D.
Capacity utilisation Value
Transport from production place to user (A4) Distance (km) Fuel/Energy Consumption Unit
(incl. return) % (Liter/tonne)
Truck, over 32 tonnes, EURO 6 (km) 53,3 % 1956 0,023 l/tkm 44,99
Truck, over 32 tonnes, EURO 6 (km) 53,3 % 300 0,023 l/tkm 6,90
Assembly (A5) Unit Value
Product loss during installation (percentage of
Units/DU 0,050
cable)
Waste, packaging, pallet, EUR wooden pallet,
single use, to average treatment (kg) - A5, inkl. 85 kg 0,0050
km transp.
Capacity utilisation Value
Transport to waste processing (C2) Distance (km) Fuel/Energy Consumption Unit
(incl. return) % (Liter/tonne)
Truck, 16-32 tonnes, EURO 6 (km) 36,7 % 85 0,043 l/tkm 3,66
Waste processing (C3) Unit Value
Copper to recycling (kg) kg 0,053
Waste treatment of plastic mixture, incineration
kg 0,020
with energy recovery and fly ash extraction (kg)
Disposal (C4) Unit Value
Landfilling of plastic mixture (kg) kg 0,030
Landfilling of copper (kg) kg 0,035
Landfilling of ashes from incineration of Plastic
kg 0,00069
mixture, process per kg ashes and residues (kg)
Benefits and loads beyond the system
Unit Value
boundaries (D)
Substitution of primary copper with net scrap (kg) kg 0,051
Substitution of thermal energy, district heating, in
MJ 0,51
Norway (MJ)
Substitution of electricity, in Norway (MJ) MJ 0,034
6 / 12
LCA: Results
The LCA results are presented below for the declared unit defined on page 2 of the EPD document.
Environmental impact
Indicator Unit A1 A2 A3 A4 A5 C1 C2 C3 C4 D
GWP-total
kg CO2 -
4,52E-01 1,09E-02 2,51E-02 2,54E-02 2,77E-02 0 1,79E-03 4,74E-02 4,00E-03 -1,28E-01
eq
GWP-fossil
kg CO2 -
4,50E-01 1,09E-02 2,35E-02 2,53E-02 2,01E-02 0 1,79E-03 4,74E-02 4,00E-03 -1,27E-01
eq
GWP-biogenic
kg CO2 -
1,18E-03 4,52E-06 1,57E-03 1,09E-05 7,53E-03 0 7,41E-07 1,03E-06 3,11E-07 -5,83E-04
eq
GWP-luluc
kg CO2 -
4,66E-04 3,89E-06 1,44E-05 7,72E-06 1,73E-05 0 6,37E-07 1,92E-07 2,67E-07 -2,34E-04
eq
kg
ODP CFC11 - 3,90E-08 2,47E-09 7,58E-09 6,11E-09 4,22E-09 0 4,06E-10 1,03E-10 2,38E-10 -2,18E-04
eq
mol H+
AP 2,04E-02 3,14E-05 8,09E-05 8,16E-05 5,77E-04 0 5,15E-06 1,04E-05 6,34E-06 -2,09E-02
-eq
EP-FreshWater kg P -eq 1,66E-04 8,72E-08 5,80E-07 2,02E-07 4,66E-06 0 1,43E-08 9,13E-09 1,24E-08 -1,41E-04
EP-Marine kg N -eq 1,38E-03 6,21E-06 1,77E-05 1,79E-05 4,27E-05 0 1,02E-06 4,96E-06 5,89E-06 -8,64E-04
mol N -
EP-Terrestial 2,03E-02 6,95E-05 1,68E-04 1,99E-04 6,03E-04 0 1,14E-05 5,09E-05 2,54E-05 -1,34E-02
eq
kg
POCP NMVOC 5,09E-03 2,66E-05 4,67E-05 7,83E-05 1,56E-04 0 4,36E-06 1,23E-05 7,96E-06 -3,63E-03
-eq
ADP- kg Sb-
2,19E-04 3,02E-07 3,71E-07 4,52E-07 5,17E-06 0 4,95E-08 5,18E-09 6,21E-09 -1,17E-04
minerals&metals1 eq
ADP-fossil1 MJ 6,70E+00 1,65E-01 1,65E+00 4,12E-01 3,70E-01 0 2,71E-02 6,51E-03 1,88E-02 -1,15E+00
WDP1 m3 3,10E+01 1,60E-01 2,50E+01 3,16E-01 2,20E+00 0 2,62E-02 4,70E-02 3,65E-01 6,26E+00
GWP-total = Global Warming Potential total; GWP-fossil = Global Warming Potential fossil fuels; GWP-biogenic = Global Warming Potential biogenic; GWP-luluc =
Global Warming Potential land use and land use change; ODP = Depletion potential of the stratospheric ozone layer; AP = Acidification potential, Accumulated
Exceedance; EP-freshwater = Eutrophication potential, fraction of nutrients reaching freshwater end compartment: EP-marine = Eutrophication potential, fraction of
nutrients reaching marine end compartment; EP-terrestrial = Eutrophication potential, Accumulated Exceedance; POCP = Formation potential of tropospheric ozone;
ADP-minerals&metals = Abiotic depletion potential for non-fossil resources; ADP-fossil = Abiotic depletion for fossil resources potential; WDP = Water (user)
deprivation potential, deprivation-weighted water consumption
"Reading example: 9,0 E-03 = 9,0*10-3 = 0,009"
*INA Indicator Not Assessed
1. The results of this environmental impact indicator shall be used with care as the uncertainties on these results are high or as there is limited experienced with the
indicator
Remarks to environmental impacts
7 / 12
Additional environmental impact indicators
Indicator Unit A1 A2 A3 A4 A5 C1 C2 C3 C4 D
PM Disease incidence 5,70E-08 6,68E-10 4,91E-10 2,33E-09 1,84E-09 0 1,10E-10 4,50E-11 1,16E-10 -4,32E-08
IRP2 kgBq U235 -eq 2,83E-02 7,22E-04 1,63E-02 1,80E-03 1,80E-03 0 1,18E-04 1,64E-05 1,13E-04 -1,65E-03
ETP-fw1 CTUe 2,50E+02 1,22E-01 5,94E-01 3,01E-01 7,40E+00 0 2,01E-02 1,00E-01 2,20E+01 -1,92E+02
HTP-c1 CTUh 4,49E-09 0,00E+00 1,80E-11 0,00E+00 1,22E-10 0 0,00E+00 3,00E-12 1,00E-12 -2,71E-09
HTP-nc1 CTUh 3,37E-07 1,33E-10 4,46E-10 2,91E-10 9,14E-09 0 2,20E-11 1,25E-10 2,40E-11 -2,32E-07
SQP1 dimensionless 5,61E+00 1,15E-01 9,68E-02 4,72E-01 2,10E-01 0 1,89E-02 1,19E-03 4,70E-02 -2,72E+00
PM = Particulate Matter emissions; IRP = Ionizing radiation – human health; ETP-fw = Eco toxicity – freshwater; HTP-c = Human toxicity – cancer effects; HTP-nc =
Human toxicity – non cancer effects; SQP = Potential Soil Quality Index (dimensionless)
"Reading example: 9,0 E-03 = 9,0*10-3 = 0,009"
*INA Indicator Not Assessed
1. The results of this environmental impact indicator shall be used with care as the uncertainties on these results are high or as there is limited experienced with the
indicator
2. This impact category deals mainly with the eventual impact of low dose ionizing radiation on human health of the nuclear fuel cycle. It does not consider effects due
to possible nuclear accidents, occupational exposure nor due to radioactive waste disposal in underground facilities. Potential ionizing radiation from the soil, from
radon and from some construction materials is also not measured by this indicator.
8 / 12
Resource use
Indicator Unit A1 A2 A3 A4 A5 C1 C2 C3 C4 D
PERE MJ 1,36E+00 2,36E-03 2,51E-01 5,18E-03 5,41E-02 0 3,88E-04 3,62E-04 1,97E-03 -7,09E-01
PERM MJ 6,94E-02 0,00E+00 0,00E+00 0,00E+00 -6,59E-02 0 0,00E+00 0,00E+00 0,00E+00 0,00E+00
PERT MJ 1,43E+00 2,36E-03 2,51E-01 5,18E-03 -1,19E-02 0 3,88E-04 3,62E-04 1,97E-03 -7,09E-01
PENRE MJ 6,05E+00 1,65E-01 1,65E+00 4,12E-01 3,23E-01 0 2,71E-02 6,51E-03 1,88E-02 -1,15E+00
PENRM MJ 6,51E-01 0,00E+00 0,00E+00 0,00E+00 2,39E-02 0 0,00E+00 -1,10E+00 0,00E+00 0,00E+00
PENRT MJ 6,70E+00 1,65E-01 1,65E+00 4,12E-01 3,47E-01 0 2,71E-02 -1,10E+00 1,88E-02 -1,15E+00
SM kg 1,53E-02 0,00E+00 0,00E+00 0,00E+00 4,28E-04 0 0,00E+00 0,00E+00 1,15E-06 3,63E-02
RSF MJ 3,57E-02 8,46E-05 1,81E-03 1,81E-04 1,13E-03 0 1,39E-05 7,78E-06 4,09E-05 3,41E-03
NRSF MJ 7,56E-04 3,02E-04 4,63E-03 6,07E-04 3,19E-04 0 4,96E-05 0,00E+00 1,34E-05 -8,24E-03
FW m3 8,31E-03 1,77E-05 1,53E-03 4,69E-05 3,90E-04 0 2,90E-06 5,50E-05 2,42E-05 -3,36E-03
PERE = Use of renewable primary energy excluding renewable primary energy resources used as raw materials; PERM = Use of renewable primary energy resources used
as raw materials; PERT = Total use of renewable primary energy resources; PENRE = Use of non renewable primary energy excluding non-renewable primary energy
resources used as raw materials; PENRM = Use of non renewable primary energy resources used as raw materials; PENRT = Total use of non renewable primary energy
resources; SM = Use of secondary materials; RSF = Use of renewable secondary fuels; NRSF = Use of non-renewable secondary fuels; FW = Net use of fresh water
"Reading example: 9,0 E-03 = 9,0*10-3 = 0,009"
*INA Indicator Not Assessed
9 / 12
End of life - Waste
Indicator Unit A1 A2 A3 A4 A5 C1 C2 C3 C4 D
HWD kg 4,96E-03 8,52E-06 3,33E-03 2,25E-05 3,73E-04 0 1,40E-06 0,00E+00 1,35E-03 -1,41E-03
NHWD kg 1,93E-01 8,03E-03 1,60E-02 3,58E-02 1,47E-02 0 1,32E-03 0,00E+00 6,67E-02 -6,09E-02
RWD kg 2,64E-05 1,12E-06 2,10E-05 2,81E-06 2,02E-06 0 1,84E-07 0,00E+00 1,29E-07 -1,47E-06
HWD = Hazardous waste disposed; NHWD = Non-hazardous waste disposed; RWD = Radioactive waste disposed
"Reading example: 9,0 E-03 = 9,0*10-3 = 0,009"
*INA Indicator Not Assessed
End of life - Output flow
Indicator Unit A1 A2 A3 A4 A5 C1 C2 C3 C4 D
CRU kg 0,00E+00 0,00E+00 0,00E+00 0,00E+00 0,00E+00 0 0,00E+00 0,00E+00 0,00E+00 0,00E+00
MFR kg 0,00E+00 0,00E+00 1,21E-02 0,00E+00 2,02E-03 0 0,00E+00 5,34E-02 2,74E-06 -1,42E-03
MER kg 0,00E+00 0,00E+00 1,43E-02 0,00E+00 5,67E-03 0 0,00E+00 2,00E-02 6,69E-08 -1,87E-04
EEE MJ 0,00E+00 0,00E+00 8,73E-03 0,00E+00 4,42E-03 0 0,00E+00 3,07E-02 4,34E-06 -4,59E-04
EET MJ 0,00E+00 0,00E+00 1,32E-01 0,00E+00 6,69E-02 0 0,00E+00 4,65E-01 6,57E-05 -6,94E-03
CRU = Components for re-use; MFR = Materials for recycling; MER = Materials for energy recovery; EEE = Exported energy electrical; EET = Exported energy thermal
"Reading example: 9,0 E-03 = 9,0*10-3 = 0,009"
*INA Indicator Not Assessed
Biogenic Carbon Content
Indicator Unit At the factory gate
Biogenic carbon content in product kg C 0,00E+00
Biogenic carbon content in accompanying packaging kg C 2,07E-03
Note: 1 kg biogenic carbon is equivalent to 44/12 kg CO2
10 / 12
Additional requirements
Greenhouse gas emissions from the use of electricity in the manufacturing phase
National production mix from import, low voltage (production of transmission lines, in addition to direct emissions and losses in grid) of applied
electricity for the manufacturing process (A3).
Electricity mix Source Amount Unit
Electricity, Norway (kWh) ecoinvent 3.6 24,33 g CO2-eq/kWh
Electricity, France (kWh) ecoinvent 3.6 94,37 g CO2-eq/kWh
Dangerous substances
The product contains no substances given by the REACH Candidate list.
Indoor environment
No effect on indoor environment.
Additional Environmental Information
Additional environmental impact indicators required in NPCR Part A for construction products
Indicator Unit A1 A2 A3 A4 A5 C1 C2 C3 C4 D
GWPIOBC kg CO2 -eq 4,59E-01 1,09E-02 2,48E-02 2,54E-02 2,04E-02 0 1,79E-03 4,73E-02 2,96E-03 -6,20E-02
GWP-IOBC: Global warming potential calculated according to the principle of instantaneous oxidation. In order to increase the transparency of biogenic carbon​
contribution to climate impact, the indicator GWP-IOBC is required as it declares climate impacts calculated according to the principle of instantaneous oxidation.​
GWP-IOBC is also referred to as GWP-GHG in context to Swedish public procurement legislation.
11 / 12
Bibliography
ISO 14025:2010. Environmental labels and declarations - Type III environmental declarations - Principles and procedures. International
Organization for Standardization.
ISO 14044:2006. Environmental management - Life cycle assessment - Requirements and guidelines. International Organization for
Standardization.
EN 15804:2012+A2:2019. Environmental product declaration - Core rules for the product category of construction products. European
Committee for Standardization.
ISO 21930:2017. Sustainability in buildings and civil engineering works - Core rules for environmental product declarations of construction
products. International Organization for Standardization.
EN 50693:2019. Product category rules for life cycle assessments of electronic and electrical products and systems. European Committee for
Standardization.
Ecoinvent v3, 2019. Allocation, cut-off by classification. Swiss Centre of Life Cycle Inventories.
Iversen et al., (2021). eEPD v2021.09, background information for EPD generator tool system verification, LCA.no. Report number: 07.21. System
verification report.
Philis et al., (2022). EPD generator for NPCR 027 part B for electrical wires and cables, background information for EPD generator application and
LCA data, LCA.no Report number: 03.22. PCR verification report.
EPD Norway (2022). NPCR Part A: Construction products and services. The Norwegian EPD foundation. Version 2.0 published 24.03.2021.
EPD Norway (2022). NPCR 027 Part B for electrical cables and wires. The Norwegian EPD foundation. Version 2.0 published 01.03.2022.
Program operator and publisher Phone: +47 977 22 020
The Norwegian EPD Foundation e-mail: post@epd-norge.no
Post Box 5250 Majorstuen, 0303 Oslo, Norway web: www.epd-norge.no
Owner of the declaration: Phone: 91597046
Lapp Norway AS e-mail: petter.dahl@lapp.com
Eikringen 11, 3036 Drammen, Norway web: no.lappgroup.com
Author of the Life Cycle Assessment Phone: +47 916 50 916
LCA.no AS e-mail: post@lca.no
Dokka 6A, 1671 Kråkerøy, Norway web: www.lca.no
Developer of EPD generator Phone: +47 916 50 916
LCA.no AS e-mail: post@lca.no
Dokka 6A, 1671 Kråkerøy, Norway web: www.lca.no
ECO Platform web: www.eco-platform.org
ECO Portal web: ECO Portal
12 / 12
