Environmental product declaration
in accordance with ISO 14025 and EN 15804+A2
EPD for aluminium crossbars – profile 7
Owner of the declaration: Program operator:
EL-tjeneste AS The Norwegian EPD Foundation
Product: Declaration number:
EPD for aluminium crossbars – profile 7 NEPD-6269-5523-EN
Declared unit: Registration number:
1 kg
NEPD-6269-5523-EN
This declaration is based on Product Category Rules:
CEN Standard EN 15804:2012+A2:2019 serves as core Issue date: 14.03.2024
PCR
The Norwegian EPD Foundation Valid to: 14.03.2029
NPCR 013:2021 Part B for Steel and aluminium
construction products EPD software:
LCAno EPD generator ID: 200020
1 / 11
General information
Product Owner of the declaration:
EPD for aluminium crossbars – profile 7 EL-tjeneste AS
Contact person: Andreas Iversen
Phone: +47 976 74 000
e-mail: info@el-tjeneste.no
Program operator: Manufacturer:
Post Box 5250 Majorstuen, 0303 Oslo, Norway EL-tjeneste AS
The Norwegian EPD Foundation Jæktsmedgata 4
Phone: +47 23 08 80 00 7725 Steinkjer, Norway
web: post@epd-norge.no
Declaration number: Place of production:
NEPD-6269-5523-EN EL-tjeneste AS
Jæktsmedgata 4
7725 Steinkjer, Norway
This declaration is based on Product Category Rules: Management system:
CEN Standard EN 15804:2012+A2:2019 serves as core PCR NS-EN ISO 14001: 2015 and NS-EN ISO 9001 : 2015
NPCR 013:2021 Part B for Steel and aluminium construction products
Statement of liability: Organisation no:
The owner of the declaration shall be liable for the underlying 925140074
information and evidence. EPD Norway shall not be liable with respect
to manufacturer information, life cycle assessment data and
evidences.​
Declared unit: Issue date:
14.03.2024
1 kg EPD for aluminium crossbars – profile 7
Declared unit with option: Valid to:
14.03.2029
A1,A2,A3,A4,A5,C1,C2,C3,C4,D
Year of study:
2022
Functional unit: Comparability:
Use phase is not considered, hence no functional unit. EPD of construction products may not be comparable if they not
comply with EN 15804 and seen in a building context.
General information on verification of EPD from EPD tools:
Independent verification of data, other environmental information Development and verification of EPD:
and the declaration according to ISO 14025:2010, § 8.1.3 and § 8.1.4. The declaration is created using EPD tool lca.tools ver EPD2022.03,
Verification of each EPD is made according to EPD-Norway’s developed by LCA.no. The EPD tool is integrated in the company's
guidelines for verification and approval requiring that tools are i) management system, and has been approved by EPD Norway.
integrated into the company's environmental management system, ii)
Developer of EPD: Zohaib Ali Saleem
the procedures for use of the EPD tool are approved by EPD-Norway,
and iii) the process is reviewed annually by an independent third Reviewer of company-specific input data and EPD: Jeroen Graafland
party verifier. See Appendix G of EPD-Norway's General Programme
Instructions for further information on EPD tools 3rd party verification of company-specific data and EPD: Børge Heggen
Johansen, Energiråd AS
Verification of EPD tool:
Approved:
Independent third party verification of the EPD tool, background data
and test-EPD in accordance with EPDNorway's procedures and
guidelines for verification and approval of EPD tools.
Third party verifier:
Håkon Hauan, CEO EPD-Norge
Alexander Borg, Asplan Viak AS
(no signature required)
2 / 11
Product
Product description:
EL-tjeneste aluminium crossbars are strong and lightweight products designed for use in power transmission and distribution grids in harsh
weather climates.
The aluminium crossbars come as a part of a modular system with various types of attachments and can be mounted on all types of poles; wood,
composite, aluminium and steel. The low weight compared to strength gives opportunities for the product to be mounted in ways that have a low
impact on surrounding environments. The products have a high expected lifetime and are fully recyclable at the end of life.
Product specification
EL-tjeneste aluminium crossbars are extruded profiles in aluminium alloy 6000-series and comes in a variety of sizes and shapes depending on
function and direction of load. Length of the crossbar and distance between pole and line attachment depends on the voltage level of the power
grid. All crossbars made by EL-tjeneste are anodized with a dark brown color, this gives a higher corrosion resistance and make them less visible in
surrounding environment. The color is UV resistant and reduces light reflection.
The results in the current EPD are given for an average of the different aluminium profiles. In order to calculate the environmental footprint of a
specific crossbar, the values in this EPD must be multiplied with the weight/length ratio and total length given in each product's datasheet.
This EPD covers crossbars that are made from aluminium profile nr. 7.
Materials Value Unit
Aluminium 1 kg
Technical data:
For more technical details , please refer to the table provided and https://www.el-tjeneste.no/
Aluminium profile Dimensions (WxH) Weight per length Alloy
P7 160x230 mm 22,255 kg/m AlMgSi 6082-T6
Market:
Main market Norway/Nordics, but can be sold to and used anywhere in the world.
Reference service life, product
80 - 100 years.
Reference service life, building or construction works
Not Applicable.
LCA: Calculation rules
Declared unit:
1 kg EPD for aluminium crossbars – profile 7
Cut-off criteria:
All major raw materials and all the essential energy is included. The production processes for raw materials and energy flows with very small
amounts (less than 1%) are not included. These cut-off criteria do not​ apply for hazardous materials and substances.
Allocation:
The allocation is made in accordance with the provisions of EN 15804. Incoming energy and water and waste production in-house is allocated
equally among all products through mass allocation. Effects of primary production of recycled materials is allocated to the main product in which
the material was used. The recycling process and transportation of the material is allocated to this analysis.
Data quality:
Specific data for the product composition are provided by the manufacturer. The data represent the production of the declared product and were
collected for EPD development in the year of study. Background data is based on EPDs according to EN 15804 and different LCA databases. The
data quality of the raw materials in A1 is presented in the table below.
Materials Source Data quality Year
Metal - Aluminium Modified ecoinvent 3.6 Database 2019
Metal - Aluminium Supplier Supplier specific 2021
3 / 11
System boundaries (X=included, MND=module not declared, MNR=module not relevant)
Construction Beyond the system
Product stage Use stage End of life stage
installation stage boundaries
A1 A2 A3 A4 A5 B1 B2 B3 B4 B5 B6 B7 C1 C2 C3 C4 D
X X X X X MND MND MND MND MND MND MND X X X X X
System boundary:
The scope of the study is cradle to gate with options, with life cycle modules of A1-A3, A4, C1-C4 and D. B1 - B7 are excluded. The study takes
into consideration the life cycle stages from the extraction of raw materials, production, processing and disposal, including all associated transport
stages. The flowchart further illustrates the different stages of the product's life cycle considered. Module D includes the loads of melting and
casting used aluminium potential benefits for the use of secondary aluminium outside the system boundary for the next product life cycle.
Additional technical information:
waR slairetam tropsnarT gnirutcafunaM tropsnarT ylbmessA e​sU ecnanetniaM riapeR tnemecalpeR tnemhsibrufeR lanoitarepO ygrene esu lanoitarepO esu retaw -eD noitcurtsnoc noitilomed tropsnarT etsaW gnissecorp lasopsiD -yrevoceR-esueR laitnetop-gnilcyceR
4 / 11
LCA: Scenarios and additional technical information
The following information describe the scenarios in the different modules of the EPD.
EL-tjeneste supplies products within the domestic market. Our focus is serving the end customers in the surrounding areas, located approximately
300 km within the production site.
A5: Assembly has not been included due to high uncertainties in the installation scenarios.
Capacity utilisation Value
Transport from production place to user (A4) Distance (km) Fuel/Energy Consumption Unit
(incl. return) % (Liter/tonne)
Truck, 16-32 tonnes, EURO 6 (km) - Europe 36,7 % 300 0,043 l/tkm 12,90
De-construction demolition (C1) Unit Value
Demolition of building per kg kg/DU 1,00
Capacity utilisation Value
Transport to waste processing (C2) Distance (km) Fuel/Energy Consumption Unit
(incl. return) % (Liter/tonne)
Truck, 16-32 tonnes, EURO 6 (km) - Europe 36,7 % 300 0,043 l/tkm 12,90
Waste processing (C3) Unit Value
Waste, Materials to recycling (kg) kg/DU 0,95
Disposal (C4) Unit Value
Waste, scrap aluminium, to landfill (kg) kg/DU 0,05
Benefits and loads beyond the system
Unit Value
boundaries (D)
Substitution of primary aluminium with net scrap kg/DU 0,95
5 / 11
LCA: Results
The LCA results are presented below for the declared unit defined on page 2 of the EPD document.
Environmental impact
Indicator Unit A1 A2 A3 A1-A3 A4 C1 C2 C3 C4 D
GWP-total
kg CO2 -
7,03E+00 3,19E-01 3,61E-02 7,39E+00 4,90E-02 1,32E-03 4,90E-02 0,00E+00 7,21E-04 -8,63E+00
eq
GWP-fossil
kg CO2 -
6,98E+00 3,19E-01 3,17E-02 7,33E+00 4,90E-02 1,32E-03 4,90E-02 0,00E+00 7,18E-04 -8,43E+00
eq
GWP-biogenic
kg C eqO2 -
3,62E-02 1,29E-04 4,07E-03 4,04E-02 2,03E-05 2,47E-07 2,03E-05 0,00E+00 2,29E-06 -3,88E-02
GWP-luluc
kg CO2 -
1,48E-02 1,18E-04 2,80E-04 1,74E-05 1,04E-07 1,74E-05 0,00E+00 2,79E-07 -1,60E-01
eq 1,52E-02
kg
ODP CFC11 - 9,29E-07 7,18E-08 2,52E-09 1,00E-06 1,11E-08 2,85E-10 1,11E-08 0,00E+00 2,01E-10 -7,12E-07
eq
AP mol H+ 4,16E-02 1,41E-03 2,47E-04 4,33E-02 1,41E-04 1,38E-05 1,41E-04 0,00E+00 5,57E-06 -5,71E-02
-eq
EP-FreshWater kg P -eq 1,50E-04 2,48E-06 2,32E-06 1,55E-04 3,92E-07 4,80E-09 3,92E-07 0,00E+00 1,30E-08 -3,26E-04
EP-Marine kg N -eq 5,39E-03 3,07E-04 3,67E-05 5,73E-03 2,79E-05 6,09E-06 2,79E-05 0,00E+00 2,00E-06 -7,21E-03
mol N -
EP-Terrestial 6,14E-02 3,42E-03 4,46E-04 3,12E-04 6,68E-05 3,12E-04 0,00E+00 2,25E-05 -7,93E-02
eq 6,53E-02
kg
POCP NMVOC 2,21E-02 1,12E-03 1,21E-04 2,33E-02 1,19E-04 1,84E-05 1,19E-04 0,00E+00 6,36E-06 -2,68E-02
-eq
ADP- kg Sb- 5,85E-05 8,46E-06 2,00E-06 6,89E-05 1,35E-06 2,02E-09 1,35E-06 0,00E+00 5,46E-09 1,30E-05
minerals&metals1 eq
ADP-fossil1 MJ 9,14E+01 4,78E+00 4,37E-01 9,66E+01 7,41E-01 1,81E-02 7,41E-01 0,00E+00 1,66E-02 -1,07E+02
WDP1 m3 8,63E+02 4,46E+00 6,26E+01 9,30E+02 7,17E-01 3,86E-03 7,17E-01 0,00E+00 4,29E-01 -4,83E+03
GWP-total = Global Warming Potential total; GWP-fossil = Global Warming Potential fossil fuels; GWP-biogenic = Global Warming Potential biogenic; GWP-luluc =
Global Warming Potential land use and land use change; ODP = Depletion potential of the stratospheric ozone layer; AP = Acidification potential, Accumulated
Exceedance; EP-freshwater = Eutrophication potential, fraction of nutrients reaching freshwater end compartment: EP-marine = Eutrophication potential, fraction of
nutrients reaching marine end compartment; EP-terrestrial = Eutrophication potential, Accumulated Exceedance; POCP = Formation potential of tropospheric ozone;
ADP-minerals&metals = Abiotic depletion potential for non-fossil resources; ADP-fossil = Abiotic depletion for fossil resources potential; WDP = Water (user)
deprivation potential, deprivation-weighted water consumption
"Reading example: 9,0 E-03 = 9,0*10-3 = 0,009"
*INA Indicator Not Assessed
1. The results of this environmental impact indicator shall be used with care as the uncertainties on these results are high or as there is limited experienced with the
indicator
Remarks to environmental impacts
6 / 11
Additional environmental impact indicators
Indicator Unit A1 A2 A3 A1-A3 A4 C1 C2 C3 C4 D
PM Disease incidence 5,19E-07 1,90E-08 4,01E-09 5,42E-07 3,00E-09 3,65E-10 3,00E-09 0,00E+00 9,60E-11 -5,89E-07
IRP2 kgBq U235 -eq 4,44E-01 2,09E-02 6,93E-03 4,72E-01 3,24E-03 7,78E-05 3,24E-03 0,00E+00 1,11E-04 -4,67E-01
ETP-fw1 CTUe 2,31E+02 3,51E+00 2,01E+00 2,37E+02 5,49E-01 9,92E-03 5,49E-01 0,00E+00 3,10E+01 -1,27E+02
HTP-c1 CTUh 2,44E-08 0,00E+00 8,40E-11 2,45E-08 0,00E+00 0,00E+00 0,00E+00 0,00E+00 1,00E-12 -2,14E-08
HTP-nc1 CTUh 3,06E-07 3,85E-09 2,20E-09 3,12E-07 6,00E-10 9,00E-12 6,00E-10 0,00E+00 2,50E-11 -2,49E-07
SQP1 dimensionless 3,71E+01 3,22E+00 6,66E-01 4,09E+01 5,18E-01 2,30E-03 5,18E-01 0,00E+00 4,66E-02 -9,17E-01
PM = Particulate Matter emissions; IRP = Ionizing radiation – human health; ETP-fw = Eco toxicity – freshwater; HTP-c = Human toxicity – cancer effects; HTP-nc =
Human toxicity – non cancer effects; SQP = Potential Soil Quality Index (dimensionless)
"Reading example: 9,0 E-03 = 9,0*10-3 = 0,009"
*INA Indicator Not Assessed
1. The results of this environmental impact indicator shall be used with care as the uncertainties on these results are high or as there is limited experienced with the
indicator
2. This impact category deals mainly with the eventual impact of low dose ionizing radiation on human health of the nuclear fuel cycle. It does not consider effects due
to possible nuclear accidents, occupational exposure nor due to radioactive waste disposal in underground facilities. Potential ionizing radiation from the soil, from
radon and from some construction materials is also not measured by this indicator.
7 / 11
Resource use
Indicator Unit A1 A2 A3 A1-A3 A4 C1 C2 C3 C4 D
PERE MJ 6,30E+01 6,67E-02 5,03E+00 6,81E+01 1,06E-02 9,82E-05 1,06E-02 0,00E+00 2,32E-03 -3,88E+01
PERM MJ 0,00E+00 0,00E+00 0,00E+00 0,00E+00 0,00E+00 0,00E+00 0,00E+00 0,00E+00 0,00E+00 0,00E+00
PERT MJ 6,30E+01 6,67E-02 5,03E+00 6,81E+01 1,06E-02 9,82E-05 1,06E-02 0,00E+00 2,32E-03 -3,88E+01
PENRE MJ 9,20E+01 4,78E+00 4,38E-01 9,72E+01 7,41E-01 1,81E-02 7,41E-01 0,00E+00 1,66E-02 -1,07E+02
PENRM MJ 0,00E+00 0,00E+00 0,00E+00 0,00E+00 0,00E+00 0,00E+00 0,00E+00 0,00E+00 0,00E+00 0,00E+00
PENRT MJ 9,20E+01 4,78E+00 7,48E-01 9,75E+01 7,41E-01 1,81E-02 7,41E-01 0,00E+00 1,66E-02 -1,07E+02
SM kg 0,00E+00 0,00E+00 0,00E+00 0,00E+00 0,00E+00 8,91E-06 0,00E+00 0,00E+00 0,00E+00 0,00E+00
RSF MJ 2,20E-01 2,37E-03 3,68E-03 2,26E-01 3,79E-04 2,41E-06 3,79E-04 0,00E+00 4,80E-05 -1,59E-02
NRSF MJ 9,37E-02 8,37E-03 3,53E-02 1,37E-01 1,36E-03 3,55E-05 1,36E-03 0,00E+00 2,24E-05 5,71E-02
FW m3 5,32E-01 4,99E-04 3,48E-02 5,67E-01 7,92E-05 9,34E-07 7,92E-05 0,00E+00 2,17E-05 -2,12E-01
PERE = Use of renewable primary energy excluding renewable primary energy resources used as raw materials; PERM = Use of renewable primary energy resources used
as raw materials; PERT = Total use of renewable primary energy resources; PENRE = Use of non renewable primary energy excluding non-renewable primary energy
resources used as raw materials; PENRM = Use of non renewable primary energy resources used as raw materials; PENRT = Total use of non renewable primary energy
resources; SM = Use of secondary materials; RSF = Use of renewable secondary fuels; NRSF = Use of non-renewable secondary fuels; FW = Net use of fresh water
"Reading example: 9,0 E-03 = 9,0*10-3 = 0,009"
*INA Indicator Not Assessed
8 / 11
End of life - Waste
Indicator Unit A1 A2 A3 A1-A3 A4 C1 C2 C3 C4 D
HWD kg 2,56E-02 2,44E-04 2,31E-04 2,61E-02 3,82E-05 5,34E-07 3,82E-05 0,00E+00 0,00E+00 3,56E-02
NHWD kg 2,79E+00 2,23E-01 8,39E-02 3,10E+00 3,60E-02 2,15E-05 3,60E-02 0,00E+00 5,00E-02 -2,45E+00
RWD kg 4,52E-04 3,26E-05 3,54E-06 4,88E-04 5,05E-06 1,26E-07 5,05E-06 0,00E+00 0,00E+00 -4,39E-04
HWD = Hazardous waste disposed; NHWD = Non-hazardous waste disposed; RWD = Radioactive waste disposed
"Reading example: 9,0 E-03 = 9,0*10-3 = 0,009"
*INA Indicator Not Assessed
End of life - Output flow
Indicator Unit A1 A2 A3 A1-A3 A4 C1 C2 C3 C4 D
CRU kg 0,00E+00 0,00E+00 0,00E+00 0,00E+00 0,00E+00 0,00E+00 0,00E+00 0,00E+00 0,00E+00 0,00E+00
MFR kg 0,00E+00 0,00E+00 5,49E-02 5,49E-02 0,00E+00 8,75E-06 0,00E+00 9,50E-01 0,00E+00 0,00E+00
MER kg 0,00E+00 0,00E+00 0,00E+00 0,00E+00 0,00E+00 2,71E-08 0,00E+00 0,00E+00 0,00E+00 0,00E+00
EEE MJ 0,00E+00 0,00E+00 0,00E+00 0,00E+00 0,00E+00 9,30E-08 0,00E+00 0,00E+00 0,00E+00 0,00E+00
EET MJ 0,00E+00 0,00E+00 0,00E+00 0,00E+00 0,00E+00 1,41E-06 0,00E+00 0,00E+00 0,00E+00 0,00E+00
CRU = Components for re-use; MFR = Materials for recycling; MER = Materials for energy recovery; EEE = Exported energy electrical; EET = Exported energy thermal
"Reading example: 9,0 E-03 = 9,0*10-3 = 0,009"
*INA Indicator Not Assessed
Biogenic Carbon Content
Indicator Unit At the factory gate
Biogenic carbon content in product kg C 0,00E+00
Biogenic carbon content in accompanying packaging kg C 0,00E+00
Note: 1 kg biogenic carbon is equivalent to 44/12 kg CO2
9 / 11
Additional requirements
Greenhouse gas emissions from the use of electricity in the manufacturing phase
National production mix from import, low voltage (production of transmission lines, in addition to direct emissions and losses in grid) of applied
electricity for the manufacturing process (A3).
Electricity mix Data source Amount Unit
Electricity ecoinvent 3.6 24,33 g CO2-eq/kWh
Dangerous substances
The product contains no substances given by the REACH Candidate list.
Indoor environment
Does not have any impact on the indoor environment. The product is externally used.
Additional Environmental Information
Additional environmental impact indicators required in NPCR Part A for construction products
Indicator Unit A1 A2 A3 A1-A3 A4 C1 C2 C3 C4 D
GWPIOBC kg CO2 -eq 7,03E+00 3,19E-01 3,27E-02 7,38E+00 4,90E-02 1,32E-03 4,90E-02 0,00E+00 7,21E-04 -8,24E+00
GWP-IOBC: Global warming potential calculated according to the principle of instantaneous oxidation. In order to increase the transparency of biogenic carbon​
contribution to climate impact, the indicator GWP-IOBC is required as it declares climate impacts calculated according to the principle of instantaneous oxidation.​
GWP-IOBC is also referred to as GWP-GHG in context to Swedish public procurement legislation.
10 / 11
Bibliography
ISO 14025:2010 Environmental labels and declarations - Type III environmental declarations - Principles and procedures.
ISO 14044:2006 Environmental management - Life cycle assessment - Requirements and guidelines.
EN 15804:2012+A2:2019 Environmental product declaration - Core rules for the product category of construction products.
ISO21930:2017 Sustainability inbuildingsand civil engineering works - Core rules for environmental productdeclarations ofconstruction
products.
ecoinvent v3, Allocation, cut-off byclassification, Swiss Centre ofLife Cycle Inventories.
Iversenetal., (2021) eEPD v2021.09 Background information for EPD generatortool systemverification, LCA.no Report number: 07.21​
Graafland and Iversen, (2022) EPD generatorfor EPD generatorfor NPCR 013 Part B for Steel and Aluminum, Background information for EPD
generatorapplication and LCA data, LCA.no report number: 08.22
​
NPCR Part A: Construction products and services. Ver. 2.0. April 2021, EPD-Norge.
​
NPCR 013 Part B for Steel and Aluminium Construction Products , Ver. 4.0, 06.10.2021, EPD Norway.
Program operator and publisher Phone: +47 23 08 80 00
The Norwegian EPD Foundation e-mail: post@epd-norge.no
Post Box 5250 Majorstuen, 0303 Oslo, Norway web: www.epd-norge.no
Owner of the declaration: Phone: +47 976 74 000
EL-tjeneste AS e-mail: info@el-tjeneste.no
https://www.el-
Jæktsmedgata 4, 7725 Steinkjer web:
tjeneste.no/
Author of the Life Cycle Assessment Phone: +47 916 50 916
LCA.no AS e-mail: post@lca.no
Dokka 6B, 1671 web: www.lca.no
Developer of EPD generator Phone: +47 916 50 916
LCA.no AS e-mail: post@lca.no
Dokka 6B,1671 Kråkerøy web: www.lca.no
ECO Platform web: www.eco-platform.org
ECO Portal web: ECO Portal
11 / 11
