Environmental product declaration
in accordance with ISO 14025 and EN 15804+A2
Firebreather Cavity Barrier 36mm 1130mm
Owner of the declaration: Program operator:
Securo AS The Norwegian EPD Foundation
Product: Declaration number:
Firebreather Cavity Barrier 36mm 1130mm
Registration number:
Declared unit:
1 pcs Issue date:
This declaration is based on Product Category Rules: Valid to:
CEN Standard EN 15804:2012+A2:2019 serves as core
EPD Software:
PCR
The Norwegian EPD Foundation LCA.no EPD generator ID: 120390
NPCR 030:2021 Part B for ventilation components
1 / 11
General information
Product Owner of the declaration:
Firebreather Cavity Barrier 36mm 1130mm Securo AS
Contact person: Ole Øivind Skjetne
Phone: +47 994 19 000
e-mail: post@securo.no
Program operator: Manufacturer:
Post Box 5250 Majorstuen, 0303 Oslo, Norway Securo AS
The Norwegian EPD Foundation
Phone: +47 23 08 80 00
web: post@epd-norge.no
Declaration number: Place of production:
Securo AS
Industriveien 10
7652 Verdal , Norway
This declaration is based on Product Category Rules: Management system:
CEN Standard EN 15804:2012+A2:2019 serves as core PCR
NPCR 030:2021 Part B for ventilation components
Statement of liability: Organisation no:
The owner of the declaration shall be liable for the underlying 990 590 079
information and evidence. EPD Norway shall not be liable with respect
to manufacturer information, life cycle assessment data and
evidences.​
Declared unit: Issue date:
1 pcs Firebreather Cavity Barrier 36mm 1130mm
Declared unit with option: Valid to:
A1-A3,A4,A5,C1,C2,C3,C4,D
Year of study:
2023
Functional unit: Comparability:
Fire separation in ventilated facade systems - 36mm Cavity depth, EPD of construction products may not be comparable if they not
CC120 - rated EI30 to EI90 (EN 13501-2). comply with EN 15804 and seen in a building context.
General information on verification of EPD from EPD tools: Development and verification of EPD:
Independent verification of data, other environmental information The declaration is created using EPD tool lca.tools ver EPD2022.03,
and the declaration according to ISO 14025:2010, § 8.1.3 and § 8.1.4. developed by LCA.no. The EPD tool is integrated in the company's
Verification of each EPD is made according to EPD-Norway’s management system and has been approved by EPD Norway.
guidelines for verification and approval requiring that tools are i)
integrated into the company's environmental management system, ii) Developer of EPD: Ole Øivind Skjetne
the procedures for use of the EPD tool are approved by EPD-Norway,
Reviewer of company-specific input data and EPD:​ Bengt Are
and iii) the process is reviewed annually by an independent third
Zakariassen
party verifier. See Appendix G of EPD-Norway's General Programme
Instructions for further information on EPD tools
Verification of EPD tool: Approved:
Independent third party verification of the EPD tool, background data
and test-EPD in accordance with EPDNorway's procedures and
guidelines for verification and approval of EPD tools.
Third party verifier:
Alexander Borg, Asplan Viak AS
(no signature required)
2 / 11
Product
Product description:
Ventilated Cavity barrier with EI 30 to EI 90 rating that instantly blocks flames, sparks and burning embers. The product enables ventilation and
drainage of water in ventilated facade systems and ventilated eaves.
For more information see our website: https://securonorway.com/products/cavity-barrier/
Product specification
The Firebreather ventilated cavity barrier stops fire & flames from entering and propagating in the cavity found in ventilated facade systems, and
ventilated eaves. The product utilizes a flame arrester principle, in combination with an intumescent material - to rapidly block the air cavity in the
event of a fire. In its normal state, the product allows air and water to pass, thus enabling ventilation and outlet of vapor and moisture from the
construction.
The product is entirely passive, and normally requires little to no maintenance over its life cycle.
The product may be returned to Securo after decommissioning for evaluation, testing and documentation to re-enter the product on the market if
found suitable.
Materials kg %
Fire retardant 0,25 33,33
Metal - Stainless steel 0,50 66,67
Total 0,75
Packaging kg %
Packaging - Wood 0,31 95,68
Recycled cardboard 0,01 4,32
Total incl. packaging 1,07
Technical data:
Lenght: 1 130 mm
Width: 36 mm
Height: 112 mm
Fire rating: EI 30 to EI 90 following EN 13501-2
Market:
Construction Onshore, Norway.
Reference service life, product
The reference service life of the product varies with the application environment.
Reference service life, building or construction works
Approx. 60 years.
LCA: Calculation rules
Declared unit:
1 pcs Firebreather Cavity Barrier 36mm 1130mm
Cut-off criteria:
All major raw materials and all the essential energy is included. The production processes for raw materials and energy flows with very small
amounts (less than 1%) are not included. These cut-off criteria do not​ apply for hazardous materials and substances.
Allocation:
The allocation is made in accordance with the provisions of EN 15804. Energy, water and waste production in-house is allocated equally among all
products through mass allocation. Effects of primary production of recycled materials is allocated to the main product in which the material was
used. The recycling process and transportation of the material is allocated to this analysis.
Data quality:
Specific data for the product composition are provided by the manufacturer. The data represent the production of the declared product and were
collected for EPD development in the year of study. Background data is based on EPDs according to EN 15804 and different LCA databases. The
data quality of the raw materials in A1 is presented in the table below.
Materials Source Data quality Year
Fire retardant ecoinvent 3.6 Database 2019
Packaging - Wood ecoinvent 3.6 Database 2019
Metal - Stainless steel Modified ecoinvent 3.6 Database 2019
Recycled cardboard Modified ecoinvent 3.6 Database 2019
3 / 11
System boundaries (X=included, MND=module not declared, MNR=module not relevant)
Construction Beyond the system
Product stage Use stage End of life stage
installation stage boundaries
A1 A2 A3 A4 A5 B1 B2 B3 B4 B5 B6 B7 C1 C2 C3 C4 D
X X X X X MNR MNR MNR MNR MNR MNR MNR X X X X X
System boundary:
The use stage has not been considered for the product, as there normally is no actions related to the use of the product after Assembly until de-
construction.
Additional technical information:
Given the system boundary of 1 pc, the Assembly is based on the assumed use of regular plasterboard or concrete screws for fixing the product. A
total of 3 screws is used pr. product.
Attentive and careful decommissioning of the product allows the product to undergo an inspection and performance test at Securo - to verify and
document its suitability for re-use as-is.
waR slairetam tropsnarT gnirutcafunaM tropsnarT ylbmessA e​sU ecnanetniaM riapeR tnemecalpeR tnemhsibrufeR lanoitarepO ygrene esu lanoitarepO esu retaw -eD noitcurtsnoc noitilomed tropsnarT etsaW gnissecorp lasopsiD -yrevoceR-esueR laitnetop-gnilcyceR
4 / 11
LCA: Scenarios and additional technical information
The following information describe the scenarios in the different modules of the EPD.
A5 & C1: installation using 3 generic metal fasteners. The power consumption of the fixing is considered negligible.
A4 & C2: Generic distances for transport in Norway.
Capacity utilisation Value
Transport from production place to user (A4) Distance (km) Fuel/Energy Consumption Unit
(incl. return) % (Liter/tonne)
Truck, 16-32 tonnes, EURO 6 (km) - Europe 36,7 % 300 0,043 l/tkm 12,90
Assembly (A5) Unit Value
Fasteners, steel screws (kg) kg/DU 0,02
Waste, Packaging cardboard, corrugated, 100 %
kg 0,01
recycled, to average treatment (kg)
Waste, Packaging pallet, wood, walls (kg) kg 0,26
Waste, packaging, pallet, EUR wooden pallet,
kg 0,05
single use, to average treatment (kg)
Capacity utilisation Value
Transport to waste processing (C2) Distance (km) Fuel/Energy Consumption Unit
(incl. return) % (Liter/tonne)
Truck, 16-32 tonnes, EURO 6 (km) - Europe 36,7 % 85 0,043 l/tkm 3,66
Waste processing (C3) Unit Value
Waste treatment per kg Non-hazardous waste,
kg 0,23
incineration with fly ash extraction - C3 (kg)
Waste, Materials to recycling (kg) kg 0,46
Disposal (C4) Unit Value
Landfilling of ashes from incineration of Non-
hazardous waste, process per kg ashes and kg 0,05
residues - C4 (kg)
Waste, non-hazardous waste, to landfill (kg) kg 0,03
Waste, scrap steel, to landfill (kg) kg 0,05
Benefits and loads beyond the system
Unit Value
boundaries (D)
Substitution of electricity, in Norway (MJ) MJ 0,13
Substitution of primary steel with net scrap kg 0,41
Substitution of thermal energy, district heating, in
MJ 2,02
Norway (MJ)
5 / 11
LCA: Results
The LCA results are presented below for the declared unit defined on page 2 of the EPD document.
Environmental impact
Indicator Unit A1-A3 A4 A5 C1 C2 C3 C4 D
GWP-total kg CO2 -eq 4,58E+00 5,27E-02 6,09E-01 0 1,49E-02 5,27E-01 2,06E-02 -4,64E-01
GWP-fossil kg CO2 -eq 5,01E+00 5,26E-02 6,67E-02 0 1,49E-02 5,27E-01 1,66E-03 -4,63E-01
GWP-biogenic kg CO2 -eq -4,54E-01 2,18E-05 5,42E-01 0 6,17E-06 0,00E+00 1,89E-02 -2,73E-04
GWP-luluc kg CO2 -eq 2,49E-02 1,87E-05 3,99E-05 0 5,31E-06 8,84E-06 1,98E-07 -6,06E-04
ODP kg CFC11 -eq 3,55E-07 1,19E-08 5,46E-09 0 3,38E-09 3,49E-09 2,40E-10 -8,54E-04
AP mol H+ -eq 3,36E-02 1,51E-04 3,52E-04 0 4,29E-05 7,52E-05 6,52E-06 -2,34E-03
EP-FreshWater kg P -eq 1,94E-04 4,20E-07 3,71E-06 0 1,19E-07 3,49E-07 1,29E-07 -2,88E-05
EP-Marine kg N -eq 6,01E-03 2,99E-05 8,54E-05 0 8,48E-06 2,81E-05 3,27E-05 -4,96E-04
EP-Terrestial mol N -eq 6,77E-02 3,35E-04 9,20E-04 0 9,48E-05 2,79E-04 2,30E-05 -5,09E-03
POCP kg NMVOC -eq 2,28E-02 1,28E-04 3,20E-04 0 3,63E-05 6,84E-05 1,19E-05 -2,36E-03
ADP-minerals&metals1 kg Sb -eq 1,73E-04 1,45E-06 1,51E-06 0 4,12E-07 1,40E-07 7,07E-09 -7,91E-06
ADP-fossil1 MJ 6,18E+01 7,96E-01 7,96E-01 0 2,25E-01 9,04E-02 1,75E-02 -3,97E+00
WDP1 m3 3,52E+00 7,70E-01 3,03E+00 0 2,18E-01 -1,54E+00 1,98E-01 2,13E+01
GWP-total = Global Warming Potential total; GWP-fossil = Global Warming Potential fossil fuels; GWP-biogenic = Global Warming Potential biogenic; GWP-luluc =
Global Warming Potential land use and land use change; ODP = Depletion potential of the stratospheric ozone layer; AP = Acidification potential, Accumulated
Exceedance; EP-freshwater = Eutrophication potential, fraction of nutrients reaching freshwater end compartment: EP-marine = Eutrophication potential, fraction of
nutrients reaching marine end compartment; EP-terrestrial = Eutrophication potential, Accumulated Exceedance; POCP = Formation potential of tropospheric ozone;
ADP-minerals&metals = Abiotic depletion potential for non-fossil resources; ADP-fossil = Abiotic depletion for fossil resources potential; WDP = Water (user)
deprivation potential, deprivation-weighted water consumption
"Reading example: 9,0 E-03 = 9,0*10-3 = 0,009"
*INA Indicator Not Assessed
1. The results of this environmental impact indicator shall be used with care as the uncertainties on these results are high or as there is limited experienced with the
indicator
Remarks to environmental impacts
6 / 11
Additional environmental impact indicators
Indicator Unit A1-A3 A4 A5 C1 C2 C3 C4 D
PM Disease incidence 3,87E-07 3,22E-09 4,83E-09 0 9,13E-10 4,23E-10 1,08E-10 -4,33E-08
IRP2 kgBq U235 -eq 1,48E-01 3,48E-03 2,89E-03 0 9,85E-04 3,53E-04 9,19E-05 5,51E-04
ETP-fw1 CTUe 2,00E+02 5,90E-01 2,54E+00 0 1,67E-01 1,39E+00 8,11E-02 -2,61E+01
HTP-c1 CTUh 5,17E-08 0,00E+00 3,68E-10 0 0,00E+00 4,30E-11 1,00E-12 -2,19E-09
HTP-nc1 CTUh 1,38E-07 6,44E-10 2,68E-09 0 1,83E-10 9,16E-10 2,00E-11 4,64E-08
SQP1 dimensionless 4,93E+01 5,57E-01 3,29E-01 0 1,58E-01 1,81E-02 5,30E-02 -1,41E+00
PM = Particulate Matter emissions; IRP = Ionizing radiation – human health; ETP-fw = Eco toxicity – freshwater; HTP-c = Human toxicity – cancer effects; HTP-nc =
Human toxicity – non cancer effects; SQP = Potential Soil Quality Index (dimensionless)
"Reading example: 9,0 E-03 = 9,0*10-3 = 0,009"
*INA Indicator Not Assessed
1. The results of this environmental impact indicator shall be used with care as the uncertainties on these results are high or as there is limited experienced with the
indicator
2. This impact category deals mainly with the eventual impact of low dose ionizing radiation on human health of the nuclear fuel cycle. It does not consider effects due
to possible nuclear accidents, occupational exposure nor due to radioactive waste disposal in underground facilities. Potential ionizing radiation from the soil, from
radon and from some construction materials is also not measured by this indicator.
7 / 11
Resource use
Indicator Unit A1-A3 A4 A5 C1 C2 C3 C4 D
PERE MJ 1,25E+01 1,14E-02 8,05E-02 0 3,23E-03 8,81E-03 1,04E-03 -1,34E+00
PERM MJ 2,47E+00 0,00E+00 -2,47E+00 0 0,00E+00 0,00E+00 0,00E+00 0,00E+00
PERT MJ 1,50E+01 1,14E-02 -7,28E-01 0 3,23E-03 8,81E-03 1,04E-03 -1,34E+00
PENRE MJ 5,79E+01 7,96E-01 7,97E-01 0 2,25E-01 1,14E-01 1,75E-02 -3,97E+00
PENRM MJ 3,94E+00 0,00E+00 0,00E+00 0 0,00E+00 -3,94E+00 0,00E+00 0,00E+00
PENRT MJ 6,18E+01 7,96E-01 7,97E-01 0 2,25E-01 -3,82E+00 1,75E-02 -3,97E+00
SM kg 6,89E-02 0,00E+00 0,00E+00 0 0,00E+00 0,00E+00 0,00E+00 0,00E+00
RSF MJ 6,19E-02 4,08E-04 3,07E-03 0 1,15E-04 2,21E-04 2,18E-05 1,61E-02
NRSF MJ 1,41E-02 1,46E-03 3,34E-02 0 4,13E-04 0,00E+00 1,45E-05 4,13E-01
FW m3 4,84E-02 8,51E-05 5,00E-04 0 2,41E-05 1,58E-04 2,10E-05 -2,20E-03
PERE = Use of renewable primary energy excluding renewable primary energy resources used as raw materials; PERM = Use of renewable primary energy resources used
as raw materials; PERT = Total use of renewable primary energy resources; PENRE = Use of non renewable primary energy excluding non-renewable primary energy
resources used as raw materials; PENRM = Use of non renewable primary energy resources used as raw materials; PENRT = Total use of non renewable primary energy
resources; SM = Use of secondary materials; RSF = Use of renewable secondary fuels; NRSF = Use of non-renewable secondary fuels; FW = Net use of fresh water
"Reading example: 9,0 E-03 = 9,0*10-3 = 0,009"
*INA Indicator Not Assessed
8 / 11
End of life - Waste
Indicator Unit A1-A3 A4 A5 C1 C2 C3 C4 D
HWD kg 5,06E-02 4,10E-05 4,73E-04 0 1,16E-05 0,00E+00 4,58E-02 -2,36E-03
NHWD kg 3,74E+00 3,87E-02 3,44E-01 0 1,10E-02 2,25E-01 8,41E-02 -1,89E-01
RWD kg 1,49E-04 5,42E-06 2,43E-06 0 1,54E-06 0,00E+00 1,35E-07 3,68E-07
HWD = Hazardous waste disposed; NHWD = Non-hazardous waste disposed; RWD = Radioactive waste disposed
"Reading example: 9,0 E-03 = 9,0*10-3 = 0,009"
*INA Indicator Not Assessed
End of life - Output flow
Indicator Unit A1-A3 A4 A5 C1 C2 C3 C4 D
CRU kg 0,00E+00 0,00E+00 0,00E+00 0 0,00E+00 0,00E+00 0,00E+00 0,00E+00
MFR kg 4,07E-02 0,00E+00 1,69E-02 0 0,00E+00 4,64E-01 0,00E+00 0,00E+00
MER kg 5,79E-09 0,00E+00 3,11E-01 0 0,00E+00 2,25E-01 0,00E+00 0,00E+00
EEE MJ 6,79E-04 0,00E+00 2,17E-01 0 0,00E+00 7,81E-05 0,00E+00 0,00E+00
EET MJ 1,03E-02 0,00E+00 3,28E+00 0 0,00E+00 1,18E-03 0,00E+00 0,00E+00
CRU = Components for re-use; MFR = Materials for recycling; MER = Materials for energy recovery; EEE = Exported energy electrical; EET = Exported energy thermal
"Reading example: 9,0 E-03 = 9,0*10-3 = 0,009"
*INA Indicator Not Assessed
Biogenic Carbon Content
Indicator Unit At the factory gate
Biogenic carbon content in product kg C 0,00E+00
Biogenic carbon content in accompanying packaging kg C 1,48E-01
Note: 1 kg biogenic carbon is equivalent to 44/12 kg CO2
9 / 11
Additional requirements
Greenhouse gas emissions from the use of electricity in the manufacturing phase
National production mix from import, low voltage (production of transmission lines, in addition to direct emissions and losses in grid) of applied
electricity for the manufacturing process (A3).
Electricity mix Data source Amount Unit
Electricity ecoinvent 3.6 24,33 g CO2-eq/kWh
Dangerous substances
The product contains no substances given by the REACH Candidate list.
Indoor environment
Additional Environmental Information
Additional environmental impact indicators required in NPCR Part A for construction products
Indicator Unit A1-A3 A4 A5 C1 C2 C3 C4 D
GWPIOBC kg CO2 -eq 5,13E+00 5,27E-02 6,77E-02 0 1,49E-02 2,84E-01 6,03E-04 -6,89E-01
GWP-IOBC: Global warming potential calculated according to the principle of instantaneous oxidation. In order to increase the transparency of biogenic carbon​
contribution to climate impact, the indicator GWP-IOBC is required as it declares climate impacts calculated according to the principle of instantaneous oxidation.​
GWP-IOBC is also referred to as GWP-GHG in context to Swedish public procurement legislation.
10 / 11
Bibliography
ISO 14025:2010 Environmental labels and declarations - Type III environmental declarations - Principles and procedures.
ISO 14044:2006 Environmental management - Life cycle assessment - Requirements and guidelines.
EN 15804:2012+A2:2019 Environmental product declaration - Core rules for the product category of construction products.
ISO 21930:2017 Sustainability in buildings and civil engineering works - Core rules for environmental product declarations of construction
products.
ecoinvent v3, Allocation, cut-off by classification, Swiss Centre of Life Cycle Inventories.
Iversen et al., (2021) eEPD v2021.09 Background information for EPD generator tool system verification, LCA.no Report number: 07.21
Graafland and Iversen (2022) EPD generator for NPCR 030 Ventilation components, Background information for EPD generator application and
LCA data, LCA.no report number: 12.22
NPCR Part A: Construction products and services. Ver. 2.0. April 2021, EPD-Norge.
NPCR 030 Part B for Ventilation components, Ver. 1.0, 18.05.2021, EPD Norway.
Securo AS, founded in 2006, is right in the center of Verdal Industrial Park, Norway. Our setup includes offices, warehousing, R&D and production
facilities, and we're proud to say that our products are "Made in Norway."
We're not just about great products; we're also all about being eco-friendly. Our products are made using clean, green energy, and we're
committed to supporting our local workforce. We're all in when it comes to sustainability.
Fire safety is a serious matter, and we take it seriously. We're always working on making things better, and that's why we're into continuous
Research and Development (R&D). Our goal is to keep pushing the boundaries and providing you with top-notch fire safety solutions. Your safety
is what drives us!
As of 2023, you'll find 12 dedicated people working here, striving for a more fire safe future.
Program operator and publisher Phone: +47 23 08 80 00
The Norwegian EPD Foundation e-mail: post@epd-norge.no
Post Box 5250 Majorstuen, 0303 Oslo, Norway web: www.epd-norge.no
Owner of the declaration: Phone: +47 994 19 000
Securo AS e-mail: post@securo.no
Industriveien 10, 7652 Verdal web: https://securonorway.com/
Author of the Life Cycle Assessment Phone: +47 916 50 916
LCA.no AS e-mail: post@lca.no
Dokka 6B, 1671 web: www.lca.no
Developer of EPD generator Phone: +47 916 50 916
LCA.no AS e-mail: post@lca.no
Dokka 6B,1671 Kråkerøy web: www.lca.no
ECO Platform web: www.eco-platform.org
ECO Portal web: ECO Portal
11 / 11
