ver1 2015
ENVIRONMENTAL PRODUCT DECLARATION
in accordance with ISO 14025, ISO 21930 and EN 15804
Owner of the declaration: Steni AS
Program operator: The Norwegian EPD Foundation
Publisher: The Norwegian EPD Foundation
Declaration number: NEPD-2581-1309-EN
Registration number: NEPD-2581-1309-EN
ECO Platform reference number: -
Issue date: 08.01.2021
Valid to: 08.01.2026
Steni Colour
Steni AS
www.epd-norge.no
NEPD-2581-1309-EN Steni Colour 1 / 8
General information
Product: Owner of the declaration:
Steni Colour Steni AS
Contact person: Herleif Rimstad
Phone: + 47 926 35 625
Program operator: e-mail: herleif.rimstad@steni.no
The Norwegian EPD Foundation
Pb. 5250 Majorstuen, 0303 Oslo Manufacturer:
Phone: +47 23 08 80 00 Steni AS
e-mail: post@epd-norge.no
Declaration number: Place of production:
NEPD-2581-1309-EN STENI AS
Lågendalsveien 2633
3277 Steinsholt
ECO Platform reference number: Norway
This declaration is based on Product Category Rules: Management system:
CEN Standard EN 15804:2012+A1:2013 serves as core ISO 9001:2015, sert. no.: 0102916
PCR and NPCR010:2019 Part B for Building boards
Statement of liability: Organisation no.:
The owner of the declaration shall be liable for the 918 150 145
underlying information and evidence. EPD-Norway shall not
be liable with respect to manufacturer information, life cycle
assessment data and evidences. Issue date: 08.01.2021
Declared unit: Valid to: 08.01.2026
1 m2 Steni Colour
Year of study:
Declared unit with option: 2020
A1,A2,A3,A4,A5,B2,C1,C2,C3,C4,D
Functional unit: Comparability:
1 m2 covering surface of installed building board with a EPD of construction products may not be comparable if
specific function, from cradle-to-grave, with activities needed they not comply with EN 15804 and seen in a building
for a study period of 60 years for the building context.
General information on verification of EPD from EPD
tools: Development and verification of EPD:
Independent verification of data, other environmental The declaration has been developed and verified using
information and the declaration according to ISO EPD tool lca.tools ver EPD2020 20, developed by
14025:2010, § 8.1.3 and § 8.1.4. Individual third party LCA.no AS. The EPD tool is integrated into the
verification of each EPD is not required when the EPD tool is company’s environmental management system, and
i)integrated into the company’s environmental management has been approved by EPD-Norway
system, ii) the procedures for use of the EPD tool are
approved by EPD-Norway, and iii) the process is reviewed Developer of the EPD:
annual. See Appendix G of EPD-Norway’s General Halgurd Shaker Sofi
Programme Instructions for further information on EPD tools.
Reviewer of company-specific input data and EPD:
Verification of EPD tool: Jan Marius Kruse
Independent third party verification of the EPD tool,
background data and test-EPD in accordance with EPD-
Norway’s procedures and guidelines for verification and Approved:
approval of EPD tools.
Michael M. Jenssen
(no signature required)
NEPD-2581-1309-EN Steni Colour
Product
Product description: Technical data:
STENI Colour is a robust stone-composite panel with STENI Colour is 6mm thick fiberglass-rainforced stone composite panel with a
a smooth surface designed for use as exterior ventilated cladding core of crushed stone, with an avrage wight of 12kg/m2. The panel comes in
on all types of buildings. The panels consist of several layers of materials various colors, sizes and glosses.
that are hardened and cured to give durability and a long-lasting
surface. The panel has SINTEF technical approval TG 2165.
Steni Colour is delivered in a wide range of colours, sizes and three gloss
Market:
variations. Low maintenance and a 60-year warranty secure low LCC.
Main markets; Europe, US, Canada, UAE.
Product specification
STENI Colour comes in various widths and lengths, with standard panel Reference service life, product
size on stock that are 1195x2995mm. The panels can also be delivered
The panel has 60 years as referance service life under normal conditions,
from 850mm to 3495mm in length and 295-1195mm in width. The
assuming installation, use and maintenance instructions are followed.
panels can also be delivered according to customers specifictions.
Reference service life, building
Materials %
Packaging 3,68 60 years
Reinforcement 4,19
Additives 0,44
Binder 18,59
Filler, core stone aggregate 72,28
Lacquer, solvent free 0,81
LCA: Calculation rules
Declared unit: Allocation:
The allocation is made in accordance with the provisions of EN 15804.
1 m2 Steni Colour
Incoming energy and water and waste production in-house is allocated
Cut-off criteria: equally among all products through mass allocation. Effects of primary
production of recycled materials is allocated to the main product in which the
All major raw materials and all the essential energy is included. The
material was used. The recycling process and transportation of the material is
production processes for raw materials and energy flows with very small
allocated to this analysis.
amounts (less than 1%) are not included. These cut-off criteria do not
apply for hazardous materials and substances.
Data quality:
Specific data for the product composition are provided by the manufacturer. They represent the production of the declared product and were collected for EPD
development in the year of study. Background data is based on registered EPDs according to EN 15804, Ostfold Research databases, ecoinvent and other LCA
databases. The data quality of the raw materials in A1 is presented in the table below.
Materials Source Data quality Year
Additives EcoInvent 3.6 Database 2016
Additives LCA.no Database 2016
Packaging ecoinvent 3.4 Database 2017
Lacquer, solvent free ecoinvent 3.5 Database 2018
Packaging NorEnviro Database 2018
Binder ecoinvent 3.6 Database 2019
Filler, core stone aggregate ecoinvent 3.6 Database 2019
Lacquer, solvent free ecoinvent 3.6 Database 2019
Reinforcement ecoinvent 3.6 Database 2019
Packaging Modified ecoinvent 3.6 Database 2019
Binder Specific data from supplier 2019 Database 2019
NEPD-2581-1309-EN Steni Colour 3 / 8
System boundary:
The analysis as shown includes "Cradel To Gate" with the modules A1-A3, and with options A4, A5, B2, C1,C2,C3 and C4.
Additional technical information:
The panel has SINTEF technical approval TG 2165
Fire class: B-S1,d0 according to EN 13501-1.
Dimentional stability: 0,04% according to EN 438-2 part 18.
Thickness: 6mm according to EN 438-2 part 5.
The product is registered in:
Sunda Hus, Byggvarubedömningen, Nordic ECO Label.
NEPD-2581-1309-EN Steni Colour 4 / 8
LCA: Scenarios and additional technical information
The following information describe the scenarios in the different modules of the EPD.
The only maintenance neaded is cleaning with water approximately every 10th year. After end of life, the panels will be taken down and sent direktly to disposal.
Transport from production place to user (A4)
Capacity utilisation Fuel/Energy
Type Type of vehicle Distance km Unit Value (l/t)
(incl. return) % consumption
Truck 38,8 % Truck, lorry 16-32 tonnes, EURO 6 300 0,043626 l/tkm 13,09
Railway l/tkm
Boat l/tkm
Other Transportation l/tkm
Assembly (A5) End of Life (C1, C3, C4)
. Unit Value . Unit Value
Auxiliary kg Hazardous waste disposed kg
Water consumption m3 Collected as mixed construction waste kg 12,0000
Electricity consumption kWh 0,0050 Reuse kg
Other energy carriers MJ Recycling kg
Material loss kg Energy recovery kg
Output materials from waste treatment kg 0,5220 To landfill kg 12,0000
Dust in the air kg
VOC emissions kg
Maintenance (B2)/Repair (B3)
. Unit Value
Maintenance cycle* .
Auxiliary kg 0,0300
Other resources kg
Water consumption m3
Electricity consumption kWh
Other energy carriers MJ
Material loss kg
VOC emissions kg
Transport to waste processing (C2)
Capacity utilisation Fuel/Energy
Type Type of vehicle Distance km Unit Value (l/t)
(incl. return) % consumption
Truck 38,8 % Truck, lorry 16-32 tonnes, EURO 6 50 0,043626 l/tkm 2,18
Railway l/tkm
Boat l/tkm
Other Transportation l/tkm
¨
Benefits and loads beyond the system boundaries (D)
. Unit Value
Substitution of thermal energy, district heating, in Norway (MJ) MJ/DU 5,04
Substitution of electricity, in Norway (MJ) MJ/DU 0,73
Substitution of primary aggregates with crushed recycled stone products (kg) kg/DU 0,07
NEPD-2581-1309-EN Steni Colour 5 / 8
LCA: Results
System boundaries (X=included, MND=module not declared, MNR=module not relevant)
Construction Beyond the
Product stage installation User stage End of life stage . system
stage bondaries
A1 A2 A3 A4 A5 B1 B2 B3 B4 B5 B6 B7 C1 C2 C3 C4 . D
X X X X X MNR X MNR MNR MNR MNR MNR X X X X . X
Environmental impact
Parameter Unit A1-A3 A4 A5 B2 C1 C2 C3 C4 D
GWP kg CO 2 -eq 1,78E+01 5,74E-01 6,17E-02 1,09E-02 1,55E-04 9,56E-02 6,64E-03 5,12E-02 -4,88E-02
ODP kg CFC11 -eq 2,46E-06 1,08E-07 2,32E-09 1,05E-09 1,50E-11 1,80E-08 1,32E-09 1,99E-08 -1,05E-08
POCP kg C 2H 4-eq 1,08E-02 8,69E-05 4,79E-06 3,47E-06 3,48E-08 1,45E-05 1,22E-06 1,29E-05 -4,47E-05
AP kg SO 2 -eq 6,26E-02 1,35E-03 1,26E-04 5,71E-05 7,25E-07 2,25E-04 3,36E-05 3,72E-04 -2,39E-04
EP kg PO 3- -eq 6,71E-03 1,77E-04 3,30E-05 7,16E-06 1,75E-07 2,95E-05 5,95E-06 7,25E-05 -6,16E-05
4
ADPM kg Sb -eq 2,45E-05 1,78E-06 3,71E-08 3,99E-08 2,54E-09 2,97E-07 4,05E-10 7,92E-10 -4,03E-07
ADPE MJ 3,16E+02 8,66E+00 2,59E-01 1,20E-01 1,57E-03 1,44E+00 6,45E-02 1,63E+00 -5,99E-01
GWP Global warming potential; ODP Depletion potential of the stratospheric ozone layer; POCP Formation potential of tropospheric photochemical oxidants;
AP Acidification potential of land and water; EP Eutrophication potential; ADPM Abiotic depletion potential for non fossil resources; ADPE Abiotic depletion
potential for fossil resources
"Reading example: 9,0 E-03 = 9,0*10-3 = 0,009"
*INA Indicator Not Assessed
waR slairetam tropsnarT gnirutcafunaM tropsnarT ylbmessA esU ecnanetniaM riapeR tnemecalpeR tnemhsibrufeR lanoitarepO ygrene esu lanoitarepO esu
retaw
-eD noitcurtsnoc noitilomed tropsnarT etsaW gnissecorp lasopsiD -yrevoceR-esueR -gnilcyceR laitnetop
NEPD-2581-1309-EN Steni Colour 6 / 8
Resource use
Parameter Unit A1-A3 A4 A5 B2 C1 C2 C3 C4 D
RPEE MJ 4,88E+01 1,28E-01 7,16E+00 2,28E-02 2,04E-02 2,13E-02 8,66E-02 2,56E-02 -2,52E+00
RPEM MJ 9,18E+00 0,00E+00 0,00E+00 0,00E+00 0,00E+00 0,00E+00 0,00E+00 0,00E+00 0,00E+00
TPE MJ 6,72E+01 1,28E-01 7,16E+00 2,28E-02 2,04E-02 2,13E-02 8,66E-02 2,56E-02 -2,52E+00
NRPE MJ 2,69E+02 8,87E+00 8,40E-01 1,84E-01 2,71E-03 1,48E+00 1,69E-01 1,66E+00 -1,36E+00
NRPM MJ 7,79E+01 0,00E+00 0,00E+00 0,00E+00 0,00E+00 0,00E+00 0,00E+00 0,00E+00 0,00E+00
TRPE MJ 3,47E+02 8,87E+00 8,40E-01 1,84E-01 2,71E-03 1,48E+00 1,69E-01 1,66E+00 -1,36E+00
SM kg 2,00E-03 0,00E+00 0,00E+00 0,00E+00 0,00E+00 0,00E+00 0,00E+00 0,00E+00 0,00E+00
RSF MJ 4,45E-03 0,00E+00 3,55E-06 0,00E+00 3,55E-06 0,00E+00 0,00E+00 0,00E+00 -1,44E-04
NRSF MJ 0,00E+00 0,00E+00 0,00E+00 0,00E+00 0,00E+00 0,00E+00 0,00E+00 0,00E+00 0,00E+00
W m3 8,38E-02 1,68E-03 1,90E-04 3,51E-02 1,13E-06 2,80E-04 4,24E-05 1,92E-03 -4,87E-04
RPEE Renewable primary energy resources used as energy carrier; RPEM Renewable primary energy resources used as raw materials; TPE Total use of renewable
primary energy resources; NRPE Non renewable primary energy resources used as energy carrier; NRPM Non renewable primary energy resources used as
materials; TRPE Total use of non renewable primary energy resources; SM Use of secondary materials; RSF Use of renewable secondary fuels; NRSF Use of non
renewable secondary fuels; W Use of net fresh water
"Reading example: 9,0 E-03 = 9,0*10-3 = 0,009"
*INA Indicator Not Assessed
End of life - Waste
Parameter Unit A1-A3 A4 A5 B2 C1 C2 C3 C4 D
HW kg 5,49E-02 5,22E-06 4,10E-07 4,73E-07 3,48E-09 8,71E-07 1,56E-07 1,85E-06 -1,27E-06
NHW kg 9,03E+00 4,75E-01 2,21E-02 6,90E-03 2,05E-04 7,92E-02 1,91E-03 1,20E+01 -2,78E-02
RW kg 6,96E-04 6,09E-05 1,33E-06 1,05E-06 1,75E-08 1,01E-05 1,78E-06 1,13E-05 -1,27E-05
HW Hazardous waste disposed; NHW Non hazardous waste disposed; RW Radioactive waste disposed
"Reading example: 9,0 E-03 = 9,0*10-3 = 0,009"
*INA Indicator Not Assessed
End of life - Output flow
Parameter Unit A1-A3 A4 A5 B2 C1 C2 C3 C4 D
CR kg 3,59E-01 0,00E+00 0,00E+00 0,00E+00 0,00E+00 0,00E+00 0,00E+00 0,00E+00 0,00E+00
MR kg 2,27E-01 0,00E+00 0,00E+00 0,00E+00 0,00E+00 0,00E+00 0,00E+00 0,00E+00 0,00E+00
MER kg 1,25E+00 0,00E+00 5,22E-01 0,00E+00 0,00E+00 0,00E+00 0,00E+00 0,00E+00 0,00E+00
EEE MJ 8,43E-01 0,00E+00 4,10E-01 0,00E+00 0,00E+00 0,00E+00 0,00E+00 0,00E+00 0,00E+00
ETE MJ 9,09E+00 0,00E+00 4,51E+00 0,00E+00 0,00E+00 0,00E+00 0,00E+00 0,00E+00 0,00E+00
CR Components for reuse; MR Materials for recycling; MER Materials for energy recovery; EEE Exported electric energy; ETE Exported thermal energy
"Reading example: 9,0 E-03 = 9,0*10-3 = 0,009"
*INA Indicator Not Assessed
NEPD-2581-1309-EN Steni Colour 7 / 8
Additional Norwegian requirements
Greenhouse gas emissions from the use of electricity in the manufacturing phase
National production mix from import, low voltage (production of transmission lines, in addition to direct emissions and losses in grid) of applied electricity for the
manufacturing process (A3).
Electricity mix Data source Amount Unit
El-mix, Norway (kWh) ecoinvent 3.4 31,04 g CO2-ekv/kWh
Dangerous substances
The product contains no substances given by the REACH Candidate list or the Norwegian priority list.
Indoor environment
Not relevant
Bibliography
ISO 14025:2010 Environmental labels and declarations - Type III environmental declarations - Principles and procedures.
ISO 14044:2006 Environmental management - Life cycle assessment - Requirements and guidelines.
EN 15804:2012+A1:2013 Environmental product declaration - Core rules for the product category of construction products.
ISO 21930:2017 Sustainability in buildings and civil engineering works - Core rules for environmental product declarations of construction products.
ecoinvent v3, Allocation, cut-off by classification, Swiss Centre of Life Cycle Inventories.
Iversen et al., (2018) eEPD v3.0 - Background information for EPD generator system. LCA.no report number 04.18
Vold, M. et al. (2020) EPD-generator for Steni AS, bakgrunnsinformasjon for verifisering, LCA.no report number 03.20
NPCR Part A: Construction products and services. Ver. 1.0. April 2017, EPD-Norge.
NPCR 010 Part B for Building Boards. Ver. 3.0 October 2019, EPD-Norge.
Program operator and publisher Phone: +47 23 08 80 00
The Norwegian EPD Foundation
Post Box 5250 Majorstuen, 0303 Oslo e-mail: post@epd-norge.no
0303 Oslo Norway web: www.epd-norge.no
Owner of the declaration Phone: + 47 926 35 625
Steni AS Fax:
Lågendalsveien 2633 e-mail: herleif.rimstad@steni.no
3277 STEINSHOLT web: www.steni.com
Author of the Life Cycle Assessment Phone: +47 916 50 916
LCA.no AS Fax:
Dokka 1C e-mail: post@lca.no
1671 Kråkerøy web: www.lca.no
Developer of EPD generator Phone: +47 916 50 916
LCA.no AS
Dokka 1C e-mail: post@lca.no
1671 Kråkerøy web: www.lca.no
NEPD-2581-1309-EN Steni Colour 8 / 8
