ver1 2015
ENVIRONMENTAL PRODUCT DECLARATION
in accordance with ISO 14025, ISO 21930 and EN 15804
Owner of the declaration: NC Nordic Care AB
Program operator: The Norwegian EPD Foundation
Publisher: The Norwegian EPD Foundation
Declaration number: NEPD-3581-2173-EN
Registration number: NEPD-3581-2173-EN
ECO Platform reference number: -
Issue date: 06.07.2022
Valid to: 06.07.2027
Jackie chair
NC Nordic Care AB
www.epd-norge.no
NEPD-3581-2173-EN Jackie Chair (ver2-020922)
1 / 8
General information
Product: Owner of the declaration:
Jackie chair
NC Nordic Care AB
Contact person: Moa Ulfsson
Phone: +46 140 38 40 60
e-mail: moa.u@ncnordiccare.se
Program operator: Manufacturer:
NC Nordic Care AB
The Norwegian EPD Foundation
Pb. 5250 Majorstuen, 0303 Oslo
Phone: +47 23 08 80 00
e-mail: post@epd-norge.no
Declaration number: Place of production:
NC Nordic Care AB
NEPD-3581-2173-EN Ydrevägen 23, Box 30 SE 573 21 Tranås
Sweden
ECO Platform reference number: Management system:
ISO 9001, ISO 14001, ISO 45001, FSC® (C010544)
This declaration is based on Product Category Rules: Organisation no:
556249-9177
CEN Standard EN 15804:2012+A1:2013 serves as core PCR
NPCR 026:2018 Part B for furniture
Statement of liability: Issue date:
The owner of the declaration shall be liable for the underlying information and 06.07.2022
evidence. EPD Norway shall not be liable with respect to manufacturer
information, life cycle assessment data and evidences. Valid to:
06.07.2027
Declared unit: Year of study:
1 Pcs Jackie chair 2021
Declared unit with option: Comparability:
A1,A2,A3,A4 EPDs from programmes other than the Norwegian EPD Foundation may not be
comparable
Functional unit: Development and verification of EPD:
1 psc, Jackie chair. The declaration has been developed and verified using EPD tool lca.tools
ver EPD2020.11, developed by LCA.no AS. The EPD tool is integrated into
the company's environmental management system, and has been
approved by EPD-Norway
General information on verification of EPD from EPD tools:
Independent verification of data, other environmental information and Developer of EPD:
the declaration according to ISO 14025:2010, § 8.1.3 and § 8.1.4. Individual
third party verification of each EPD is not required when the EPD tool is i) Moa Ulfsson
integrated into the company's environmental management system, ii) the
procedures for use of the EPD tool are approved by EPDNorway, and iii) Reviewer of company-specific input data and EPD:
the proccess is reviewed annualy. See Appendix G of EPD-Norway's
General Programme Instructions for further information on EPD tools. Jan Jismyr
Verification of EPD tool: Approved:
Independent third party verification of the EPD tool, background data
Sign
and test-EPD in accordance with EPDNorway's procedures and guidelines
for verification and approval of EPD tools.
Erik Svanes, Norsus AS
(no signature required) Håkon Hauan, CEO EPD-Norge
Key environmental indicators Unit Cradle to gate A1 - A3
Global warming kg CO2 eqv 18,67
Total energy use MJ 466,73
Amount of recycled materials % 18,56
NEPD-3581-2173-EN Jackie Chair (ver2-020922)
2 / 8
Product
Market: Technical data:
Total weight: 5,34 kg (packaging excluded)
Mainly Europe, but is available world wide.
Total weight: 7,14 kg (packing included)
Product description:
Reference service life, product
Jackie is a versatile family of easy chairs, sofas and chairs with different
features and sizes, as well as tactile materials for variety, while 15 years service life, 5 years warrant if no other indicated.
maintaining an overall harmonious look.
Reference service life, building
The Jackie chair has been designed to meet all the identified needs of a
care chair. It is a suspendable, stackable and sound absorbent armchair
for easier cleaning, versatile furnishing and a good acoustic
environment when required.
It is available in different widths and heights to suit different individuals,
has a stable and non-tip full-length armrest with a grip on the back for
support.
For more information please visit our webpage:
https://www.ncnordiccare.se/produkter/jackie-131/
Product specification
Jackie 131
Stackable chair. Frame made of solid wood and seat and back in
plywood and veneer.
The chair are available in a few different
materials and colours. This EPD is valid for the following options:
- Frame in solid wood, available in birch (FSC Mix) or oak (FSC Mix).
- Clear lacquer, stained black or white. Other colours on request.
For other options, see variants.
Read more under "additional information" on page 4
Recycled share in Recycled share in
Materials kg %
material (kg) material (%)
Wood - Solid beech/birch 3,70 66,07 0,00 0,00
Wood - Plywood 1,08 19,29 0,00 0,00
Glue for wood 0,21 3,75 0,00 0,00
Lacquer, water based 0,05 0,89 0,00 0,00
Wood - Veneer 0,56 10,00 0,00 0,05
Total: 5,60 0,00
Recycled share in Recycled share in
Packaging kg
material (kg) material (%)
Packaging - Cardboard 1,80 1,37 76,30
Total including packaging 7,4 1,37
LCA: Calculation rules
Declared unit: Allocation:
The allocation is made in accordance with the provisions of EN 15804. Effects
1 Pcs Jackie chair
of primary production of recycled materials is allocated to the main product
Cut-off criteria: in which the material was used. The recycling process and transportation of
the material is allocated to this analysis.
All major raw materials and all the essential energy is included. The
production processes for raw materials and energy flows with very small
amounts (less than 1%) are not included. These cut-off criteria do not
apply for hazardous materials and substances.
Data quality:
Specific data for the product composition are provided by the manufacturer. They represent the production of the declared product and were collected for
EPD development in the year of study. Background data is based on registered EPDs according to EN 15804, Ostfold Research databases, ecoinvent and other
LCA databases. The data quality of the raw materials in A1 is presented in the table below.
Materials Source Data quality Year
Glue for wood ecoinvent 3.4 Database 2017
Lacquer, water based ecoinvent 3.4 Database 2017
Packaging - Cardboard ecoinvent 3.4 Database 2017
Wood - Plywood ecoinvent 3.4 Database 2017
Wood - Solid beech/birch ecoinvent 3.4 Database 2017
Wood - Veneer S-P-00172 EPD 2017
Glue for wood NORSUS Database 2020
NEPD-3581-2173-EN Jackie Chair (ver2-020922)
3 / 8
System boundary:
Additional technical information:
Jackie is tested according to EN 16139:2013 Furniture – Strength, durability and safety – Requirements for non-domestic seating.
The product is FSC® -labelled in the following executions:
Birch and oak.
Jackie has been certified according to Swedish Möbelfakta requirements. Möbelfakta is a type 1 eco-label according to ISO 14024 for furniture that considers
both quality, environment, and responsible supply chains.
https://www.mobelfakta.se/Details.html?id=1030
Continue from page 3
Dimensions:
Height 83 cm
Width 50 cm
Depth 57 cm
Seat height 46 cm
Seat depth 38 cm
Variants
Jackie 131 with upholstered seat and back.
Fabric chosen by customer, HR-foam.
Dimensions:
Height 83 cm
Width 50 cm
Depth 57 cm
Seat height 46 cm
Seat depth 38 cm
Jackie 132
Stackable chair with armrests.
Dimensions:
Height 83 cm
Width 57 cm
Depth 57 cm
Seat height 46 cm
Seat depth 38 cm
Arm height 66 cm
Jackie 132 with upholstered seat and back.
Fabric chosen by customer, HR-foam.
Dimensions:
Height 83 cm
Width 57 cm
Depth 57 cm
Seat height 46 cm
Seat depth 38 cm
Arm height 66 cm
NEPD-3581-2173-EN Jackie Chair (ver2-020922)
4 / 8
LCA: Scenarios and additional technical information
The following information describe the scenarios in the different modules of the EPD.
At our site in Tranås, we only use electricity from renewable sources. A4 transport includes transport from NC Nordic Care, Tranås to Kinnarp (140km).
Transport from production place to user (A4)
Capacity utilisation Fuel/Energy
Type Type of vehicle Distance km Unit Value (l/t)
(incl. return) % consumption
Truck 38,8 % Truck, 16-32 tonnes, EURO 6 165 0,043626 l/tkm 7,20
Railway l/tkm
Boat 50,0 % Ship, Ferry transport (kgkm) 400 0,033522 l/tkm 13,41
Other Transportation l/tkm
NEPD-3581-2173-EN Jackie Chair (ver2-020922)
5 / 8
LCA: Results
The LCA results are presented below for the declared unit defined on page 2 of the EPD document.
System boundaries (X=included, MND=module not declared, MNR=module not relevant)
Construction Beyond the
Product stage installation User stage End of life stage . system
stage bondaries
A1 A2 A3 A4 A5 B1 B2 B3 B4 B5 B6 B7 C1 C2 C3 C4 . D
X X X X MND MND MND MND MND MND MND MND MND MND MND MND . MND
Environmental impact
Parameter Unit A1 A2 A3 A4
GWP kg CO 2 -eq 3,03E+00 2,40E-01 1,54E+01 7,07E-01
ODP kg CFC11 -eq 3,63E-07 4,51E-08 8,53E-07 1,27E-07
POCP kg C 2H 4-eq 1,25E-03 3,74E-05 2,96E-03 2,34E-04
AP kg SO 2 -eq 1,33E-02 6,12E-04 7,42E-02 7,77E-03
EP kg PO 3- -eq 3,00E-03 7,91E-05 9,80E-03 9,46E-04
4
ADPM kg Sb -eq 1,90E-05 7,38E-07 2,50E-05 1,47E-06
ADPE MJ 4,45E+01 3,62E+00 1,71E+02 1,02E+01
GWP Global warming potential; ODP Depletion potential of the stratospheric ozone layer; POCP Formation potential of tropospheric photochemical oxidants;
AP Acidification potential of land and water; EP Eutrophication potential; ADPM Abiotic depletion potential for non fossil resources; ADPE Abiotic depletion
potential for fossil resources
Reading example: 9,0 E-03 = 9,0*10-3 = 0,009
*INA Indicator Not Assessed
waR slairetam tropsnarT gnirutcafunaM tropsnarT ylbmessA esU ecnanetniaM riapeR tnemecalpeR tnemhsibrufeR lanoitarepO ygrene esu lanoitarepO esu
retaw
-eD noitcurtsnoc noitilomed tropsnarT etsaW gnissecorp lasopsiD -yrevoceR-esueR -gnilcyceR laitnetop
NEPD-3581-2173-EN Jackie Chair (ver2-020922)
6 / 8
Resource use
Parameter Unit A1 A2 A3 A4
RPEE MJ 6,84E+01 5,32E-02 3,95E+01 1,24E-01
RPEM MJ 1,13E+02 0,00E+00 0,00E+00 0,00E+00
TPE MJ 1,82E+02 5,32E-02 3,95E+01 1,24E-01
NRPE MJ 5,05E+01 3,70E+00 3,05E+02 1,04E+01
NRPM MJ 2,39E-02 0,00E+00 0,00E+00 0,00E+00
TRPE MJ 5,05E+01 3,70E+00 3,05E+02 1,04E+01
SM kg 1,37E+00 0,00E+00 0,00E+00 0,00E+00
RSF MJ 0,00E+00 0,00E+00 5,34E-03 0,00E+00
NRSF MJ 0,00E+00 0,00E+00 0,00E+00 0,00E+00
W m3 7,69E-02 6,97E-04 2,60E-01 1,65E-03
RPEE Renewable primary energy resources used as energy carrier; RPEM Renewable primary energy resources used as raw materials; TPE Total use of renewable
primary energy resources; NRPE Non renewable primary energy resources used as energy carrier; NRPM Non renewable primary energy resources used as
materials; TRPE Total use of non renewable primary energy resources; SM Use of secondary materials; RSF Use of renewable secondary fuels; NRSF Use of non
renewable secondary fuels; W Use of net fresh water
Reading example: 9,0 E-03 = 9,0*10-3 = 0,009
*INA Indicator Not Assessed
End of life - Waste
Parameter Unit A1 A2 A3 A4
HW kg 7,08E-04 2,19E-06 3,58E-04 6,97E-06
NHW kg 9,62E-01 1,97E-01 3,72E+00 4,07E-01
RW kg INA* INA* INA* INA*
HW Hazardous waste disposed; NHW Non hazardous waste disposed; RW Radioactive waste disposed
Reading example: 9,0 E-03 = 9,0*10-3 = 0,009
*INA Indicator Not Assessed
End of life - Output flow
Parameter Unit A1 A2 A3 A4
CR kg 8,25E-02 0,00E+00 0,00E+00 0,00E+00
MR kg 0,00E+00 0,00E+00 1,80E+00 0,00E+00
MER kg 0,00E+00 0,00E+00 0,00E+00 0,00E+00
EEE MJ INA* INA* INA* INA*
ETE MJ INA* INA* INA* INA*
CR Components for reuse; MR Materials for recycling; MER Materials for energy recovery; EEE Exported electric energy; ETE Exported thermal energy
Reading example: 9,0 E-03 = 9,0*10-3 = 0,009
*INA Indicator Not Assessed
NEPD-3581-2173-EN Jackie Chair (ver2-020922)
7 / 8
Additional Norwegian requirements
Greenhouse gas emissions from the use of electricity in the manufacturing phase
National production mix from import, low voltage (production of transmission lines, in addition to direct emissions and losses in grid) of applied electricity for the manufacturing
process (A3).
Electricity mix Data source Amount Unit
El-mix, Sweden (kWh) ecoinvent 3.4 Alloc Rec 42,67 g CO2-ekv/kWh
Energy, electricity, European average: 1 kWh ecoinvent 3.4 594,20 g CO2-ekv/kWh
Dangerous substances
The product contains substances given by the REACH Candidate list and the Norwegian priority list that are less than 0,1 % by weight.
Indoor environment
The product is low-emitting and tested according to Swedish Möbelfakta.
Additional environmental information
Key environmental indicators for variants for this EPD: Cradle to Gate analyse from A1 to A3
Global warming (kg Share of recycled
Variant number Total energy use (MJ)
CO2) material in product(%)
Jackie chair, upholstered 30,43 696,88 0,26
Jackie armchair 20,19 487,64 0,21
Jackie armchair, upholstered 31,97 717,98 0,27
Bibliography
ISO 14025:2010 Environmental labels and declarations - Type III environmental declarations - Principles and procedures.
ISO 14044:2006 Environmental management - Life cycle assessment - Requirements and guidelines.
EN 15804:2012+A1:2013 Environmental product declaration - Core rules for the product category of construction products.
ISO 21930:2017 Sustainability in buildings and civil engineering works - Core rules for environmental product declarations of construction products.
ecoinvent v3, Allocation, cut-off by classification, Swiss Centre of Life Cycle Inventories.
Iversen et al., (2018) eEPD v3.0 - Background information for EPD generator system. LCA.no report number 04.18
Vold et al., (2019) EPD generator for Norsk Industri, Background information for industry application and LCA data, LCA.no report number 06.19.
NPCR Part A: Construction products and services. Ver. 1.0. April 2017, EPD-Norge.
NPCR 026 Part B for Furniture. Ver. 2.0 October 2018, EPD-Norge.
Program operator and publisher Phone: +47 23 08 80 00
The Norwegian EPD Foundation e-mail: post@epd-norge.no
Post Box 5250 Majorstuen, 0303 Oslo,Norway web: www.epd-norge.no
Owner of the declaration Phone: +46 140 38 40 60
NC Nordic Care AB e-mail: moa.u@ncnordiccare.se
Ydrevägen 23, Box 30 SE 573 21 Tranås web: www.ncnordiccare.se
Author of the Life Cycle Assessment Phone: +47 916 50 916
LCA.no AS e-mail: post@lca.no
Dokka 6B 1671 Kråkerøy web: www.lca.no
Developer of EPD generator Phone: +47 916 50 916
LCA.no AS e-mail: post@lca.no
Dokka 1C 1671 Kråkerøy web: www.lca.no
NEPD-3581-2173-EN Jackie Chair (ver2-020922)
8 / 8
