Environmental Product Declaration
In accordance with ISO14025:2006 and EN15804:2012+A2:2019
Welded and Pickled Stainless Steel Products
Owner of the declaration: Program holder and publisher:
Øglænd System AS The Norwegian EPD foundation
Product name: Declaration number:
Welded and Pickled Stainless Steel NEPD-7969-7623-EN
Products
Registration number:
Declared unit: NEPD-7969-7623-EN
1kg of Welded and Pickled Stainless Steel
Products Issue date: 30.10.2024
Product category /PCR: Valid to: 30.10.2029
NPCR PART A and NPCR 013 Part B
The Norwegian for Steel and Aluminum Construction
Products (references to EN15804+A2).
EPD Foundation
General information
Product: Owner of the declaration:
Welded and Pickled Stainless Steel Products Øglænd System AS
Contact person: Cecilie Vagle
Phone: (+47) 92615525
Program operator:
e-mail: cecilie.vagle@oglaend-system.com
The Norwegian EPD Foundation
Post Box 5250 Majorstuen, 0303 Oslo, Norway
Manufacturer:
Tlf: +47 23 08 80 00
e-mail: post@epd-norge.no Øglænd System AS
Klepp, Norway
Phone: (+47) 51 78 81 00
Declaration number:
e-mail: oglaend@oglaend-system.com
NEPD-7969-7623-EN
Place of production:
This declaration is based on Product Category
Øglænd System AS, Engelsvollvegen 264, 4353 Klepp St.,
Rules:
Norway
NPCR PART A and NPCR 013 Part B for Steel and
Aluminum Construction Products (references to
Management system:
EN15804+A2).
NS-EN ISO 9001:2015
Statement of liability:
NS-EN ISO 14001:2015
The owner of the declaration shall be liable for the NS-ISO 45001:2018
underlying information and evidence. EPD Norway shall not EN1090-1:2009+A1:2011Organisation no:
be liable with respect to manufacturer, life cycle assessment
NO 985 748 128 MVA
data and evidences.
Issue date:
Declared unit:
30.10.2024
1 kg of Welded and Pickled Stainless Steel Products
Valid to:
Declared unit with option:
30.10.2029
1 kg of Welded and Pickled Stainless Steel Products
with options (A4, C1, C2, C3, C4, & D)
Year of study:
[xxxx]
Functional unit:
N/A
Comparability:
Verification: EPD of construction products may not be able to compare
Independent verification of the declaration and data, if they do not comply with EN 15804 and are seen in a
according to ISO14025:2010 building context.
Internal ☐ External ☒
The EPD has been worked out by:
Modi Michael Elisa | Energiråd AS
Silvia Vilčeková
Independent verifier approved by EPD Norway Approved
Manager of EPD Norway
EPD for the best environmental decision 2
Product
Product description
Øglænd System AS provides a wide range of products including multi discipline support, cable ladders,
cable trays and accessories for low and high voltage cable management, tubing and instrumentation,
piping and HVAC across industries such as Offshore oil and gas, renewable energies, power and
distribution, ship building and infrastructure.
Product specification
This EPD covers the products from Øglænd System AS that are made from stainless steel, and then
machined, welded, and pickled. Stainless steel forms a protective chromium oxide layer when the alloy is
exposed to air, hindering direct contact between the alloy and the corrosive environment. If a stainless
steel component is damaged, a new chromium oxide layer forms, effectively resealing the damaged area.
The steel grade used for these products is AISI 316L
Tabell 1 Products covered by this EPD
Item Group no. Name/ Designation
111 111 SPB-RF CableTray System
120 120 Mekano Support System
121 121 Mekano Support System - Starter Brackets
130 130 UNO Support System
140 140 Other Support - Perforated Profiles
141 141 Other Support - Accessories
156 156 SmartCleat Cable Cleats
170 170 Equipment Rack, Stand, Tower and Brackets
171 171 Light Fitting Support - Floodlights and Handrails
199 199 No Discount Other Products
Product manufacturing
The manufacturing of these products comprises the cutting, punching, forming, and welding of the steel
input. In addition, these products are ”pickled and passivated”. This is a process to remove the heat tint
that is created during welding. The heat tint is produced by an increase in the density of chromium at the
surface and a corresponding decrease in the area below. As a result, the affected region is vulnerable to
corrosion and less aesthetically pleasing. This is efficiently solved through ”pickling and passivation”,
which cleans the area and allows a new protective chromium oxide layer to be established. The products
covered by this EPD are produced by Øgland System AS at their production site in Klepp, Norway
Tabell 2 Material input (s) used to manufacture the included products
Materials Value %
Stainless steel with alloys 1.00 100.00
Market
Worldwide.
Reference service life, product
Not relevant for cradle to gate with options
Reference service life, building
Not relevant
EPD for the best environmental decision 3
LCA: Calculation rules
Declared unit
1 kg Welded and Pickled Stainless Steel Products
Cut-off criteria
All major raw materials and all the essential energy are included. The production process for raw materials
and energy flows that are included with very small amounts (<1%) are not included. This cut-off rule
does not apply for hazardous materials and substances.
Allocation
The allocation of energy and ancillary material during production was determined by recorded production
time for the different product groups. Waste was allocated using total waste streams from the factory and
adjusted for the different product groups using mass allocation.
Data quality
General requirements and guidelines concerning use of generic and specific data and the quality of those
are as described in EN 15804: 2012, clause 6.3.6 and 6.3.7. The data is representative of temporal,
geographical and technological requirements.
Data for use in module A3 is supplied by the manufacturer and consists of the recorded amount of
specific material and energy consumption for the products studied. Specific data has been collected in
2017-2018. Generic data has been created or updated within the last 10 years, except for minor
exceptions for generic data used that are slightly older than 10 years.
The geographic region of the production sites included in the calculation is Europe. The specific data
from manufacturer is from one site, so no average data is used for several sites.
Data represents technology in use. All generic (background) data has been gathered from version 3.9.1 of
the Ecoinvent database (2023).
EPD for the best environmental decision 4
Tabell 3 System boundaries (X=included, MND=module not declared, MNR=module not relevant)
Benefits
& loads
Assembly beyond
Product stage Use stage End of life stage
stage system
boundar
y
EPD for the best environmental decision 5
slairetam
waR
tropsnarT
gnirutcafunaM
tropsnarT ylbmessA
esU
ecnanetniaM
riapeR
tnemecalpeR tnemhsibrufeR
esu
ygrene
lanoitarepO
esu
retaw
lanoitarepO
noitilomed
noitcurtsnoc-eD
tropsnarT
gnissecorp
etsaW
lasopsiD
-gnilcyceR-yrevoceR-esueR
laitnetop
A1 A2 A3 A4 A5 B1 B2 B3 B4 B5 B6 B7 C1 C2 C3 C4 D
MN MN MN MN MN MN MN MN
X X X X X X X X X
D D D D D D D D
Figur 1 System boundary
LCA: Scenarios and additional technical information
The scenarios in the different modules beyond the cradle-to-gate are described as follows:
Transport from production place to assembly/user (A4)
Transport from production place Capacity utilisation Fuel/Energy
Distance (km) Unit Value
to assembly/user (A4) (incl. return) % consumption
l/t*km,
Truck 53% 300 0.0436 13.08
diesel
End of Life (C1, C3, C4)
Unit Value
Hazardous waste disposed kg 0
Collected as mixed construction waste kg 0.02
Reuse kg 0
Recycling kg 0.98
Energy recovery kg 0
To landfill kg 0.02
C1 – dismantling is assumed to be done by use of electrical tools. . C2 – the collected mixed waste and
sorted waste are transported by truck to landfill and waste processing facility, respectively. C3 – 98% of
the product is recycled by remelting process to produce secondary aluminum billets, and C4 – 2% of the
product is collected as mixed waste and landfilled.
Transport to waste processing (C2)
Transport from production Capacity
Distance Fuel/Energy
place utilisation Unit Value
(km) consumption
to assembly/user (C2) (incl. return) %
l/t*km,
Truck 37% 20 0.0436 0.872
diesel
Benefits and loads beyond the system boundaries (D)
Benefits and loads beyond the system boundaries (D) Unit Value
Recycled stainless steel scrap kg 0.98
Substitution of primary stainless steel with net scrap kg 0.88
EPD for the best environmental decision 6
LCA: Results
The environmental performance indicators for Welded and Pickled Stainless Steel Products is shown in
the following tables. For stages A1-A3 the results are aggregated.
Core environmental impact indicators
Indicator Unit A1-A3 A4 C1 C2 C3 C4 D
GWP - total kg CO2 eq 5.32E+00 3.01E-02 6.21E-02 2.03E-03 7.79E-04 9.58E-05 -1.71E+00
GWP - fossil kg CO2 eq 5.26E+00 3.00E-02 6.21E-02 2.03E-03 7.78E-04 9.51E-05 -1.23E+00
GWP - biogenic kg CO2 eq 5.17E-02 2.30E-05 1.34E-05 7.12E-07 6.30E-07 6.94E-07 5.07E-03
GWP - luluc kg CO2 eq 5.22E-03 1.47E-05 6.99E-06 1.04E-06 1.85E-07 1.30E-08 -2.87E-04
ODP kg CFC11 eq 1.44E-07 6.82E-10 9.88E-10 3.45E-11 5.79E-12 1.54E-12 -3.05E-08
AP molc H+ eq 3.20E-02 7.44E-05 5.76E-04 5.57E-06 6.01E-06 8.69E-07 -4.58E-03
EP- freshwater kg P eq 1.35E-03 2.19E-01 3.89E-01 1.63E-02 2.31E-03 5.96E-04 -3.48E+00
EP -marine kg N eq 5.02E-03 2.03E-05 2.67E-04 1.46E-06 7.68E-07 4.01E-07 -1.13E-03
EP - terrestrial molc N eq 5.51E-02 2.08E-04 2.90E-03 1.52E-05 8.18E-06 4.36E-06 -1.20E-02
POCP kg NMVOC eq 1.90E-02 1.21E-04 8.59E-04 8.02E-06 2.52E-06 1.29E-06 -6.74E-03
ADP-M&M2 kg Sb-Eq 2.37E-03 8.61E-08 2.22E-08 5.84E-09 7.16E-10 5.24E-11 4.79E-07
ADP-fossil2 MJ 5.26E+00 4.59E-01 8.19E-01 3.09E-02 7.68E-03 1.33E-03 -1.30E+01
WDP2 m3 1.54E+00 2.36E-03 2.03E-03 1.55E-04 2.23E-04 1.55E-05 -4.98E-02
GWP-total: Global Warming Potential; GWP-fossil: Global Warming Potential fossil fuels; GWP-biogenic: Global Warming Potential biogenic; GWP-
LULUC: Global Warming Potential land use and land use change; ODP: Depletion potential of the stratospheric ozone layer; AP: Acidification potential,
Accumulated Exceedance; EP-freshwater: Eutrophication potential, fraction of nutrients reaching freshwater end compartment; See “additional Norwegian
requirements” for indicator given as PO4 eq. EP-marine: Eutrophication potential, fraction of nutrients reaching freshwater end compartment; EP-terrestrial:
Eutrophication potential, Accumulated Exceedance; POCP: Formation potential of tropospheric ozone; ADP-M&M: Abiotic depletion potential for non-fossil
resources (minerals and metals); ADP-fossil: Abiotic depletion potential for fossil resources; WDP: Water deprivation potential, deprivation weighted water
consumption
Reading example: 9,0 E-03 = 9,0*10-3 = 0,009
Additional environmental impact indicators
Indicator Unit A1-A3 A4 C1 C2 C3 C4 D
PM Disease incidence 2.96E-07 2.97E-09 1.61E-08 2.01E-10 6.48E-11 2.44E-11 -1.28E-07
IRP1 kBq U235 eq. 4.96E-01 5.75E-04 3.86E-04 2.81E-05 1.40E-05 5.98E-06 -3.61E-02
ETP-fw2 CTUe 1.67E+01 2.19E-01 3.89E-01 1.63E-02 2.31E-03 5.96E-04 -6.15E+00
HTP-c2 CTUh 2.17E-08 1.34E-11 1.91E-11 9.05E-13 2.35E-13 2.99E-14 -1.05E-08
HTP-nc2 CTUh 8.82E-08 3.28E-10 1.34E-10 2.24E-11 7.76E-12 2.36E-13 -1.90E-08
SQP2 Dimensionless 2.28E+01 6.13E-05 4.39E-05 4.26E-06 9.09E-06 3.57E-07 -4.03E-03
PM: Particulate matter emissions; IRP: Ionizing radiation, human health; ETP-fw: Ecotoxicity (freshwater); ETP-c: Human toxicity, cancer effects; HTP-nc:
Human toxicity, non-cancer effects; SQP: Land use related impacts / soil quality
1 This impact category deals mainly with the eventual impact of low dose ionizing radiation on human health of the nuclear fuel cycle. It does
not consider effects due to possible nuclear accidents, occupational exposure nor due to radioactive waste disposal in underground facilities.
Potential ionizing radiation from the soil, from radon and from some construction materials is also not measured by this indicator.
2 The results of this environmental impact indicator shall be used with care as the uncertainties on these results are high or as there is limited
experienced with the indicator
EPD for the best environmental decision 7
Resource use
Parameter Unit A1-A3 A4 C1 C2 C3 C4 D
RPEE MJ 1.29E+01 6.67E-03 4.63E-03 3.88E-04 1.87E-03 1.08E-04 -1.15E-01
RPEM MJ 0.00E+00 0.00E+00 0.00E+00 0.00E+00 0.00E+00 0.00E+00 0.00E+00
TPE MJ 1.29E+01 6.67E-03 4.63E-03 3.88E-04 1.87E-03 1.08E-04 -1.15E-01
NRPE MJ 7.10E+01 3.96E-04 3.89E-04 1.94E-05 9.80E-01 4.66E-06 -1.21E+00
NRPM MJ 1.77E+00 3.99E-02 7.48E-02 2.65E-03 2.62E-04 1.14E-04 -1.73E-01
TRPE MJ 7.28E+01 4.59E-01 8.19E-01 3.09E-02 7.68E-03 1.33E-03 -1.30E+01
SM kg 1.03E+00 4.60E-04 4.73E-04 2.34E-05 6.09E-06 4.92E-06 -2.10E-01
RSF MJ 7.67E-02 1.12E-04 5.22E-05 3.21E-06 2.39E-06 2.54E-06 -2.30E-03
NRSF MJ 5.44E-01 2.33E-04 1.41E-04 1.19E-05 1.41E-03 9.80E-07 -6.72E-03
W m3 7.46E-02 6.13E-05 4.39E-05 4.26E-06 9.09E-06 3.57E-07 -1.25E-03
RPEE Renewable primary energy resources used as energy carrier; RPEM Renewable primary energy resources used as raw materials; TPE Total use of renewable
primary energy resources; NRPE Nonrenewable primary energy resources used as energy carrier; NRPM Nonrenewable primary energy resources used as materials;
TRPE Total use of non-renewable primary energy resources; SM Use of secondary materials; RSF Use of renewable secondary fuels; NRSF Use of non-renewable
secondary fuels; W Use of net fresh water.
End of life – Waste
Parameter Unit A1-A3 A4 C1 C2 C3 C4 D
HW kg 7.35E+00 4.31E-04 6.81E-04 3.43E-05 1.40E-05 1.08E-06 5.88E-02
NHW kg 1.13E+00 3.95E-02 5.05E-04 2.64E-03 1.29E-05 2.00E-02 4.16E-02
RW kg 1.58E-04 1.39E-07 8.91E-08 6.69E-09 3.30E-09 1.34E-09 -3.05E-06
HW Hazardous waste disposed; NHW Non-hazardous waste disposed; RW Radioactive waste disposed.
End of life – output flow
Parameter Unit A1-A3 A4 C1 C2 C3 C4 D
CR kg 0.00E+00 0.00E+00 0.00E+00 0.00E+00 0.00E+00 0.00E+00 0.00E+00
MR kg 5.00E-02 0.00E+00 0.00E+00 0.00E+00 9.80E-01 0.00E+00 0.00E+00
MER kg 0.00E+00 0.00E+00 0.00E+00 0.00E+00 0.00E+00 0.00E+00 0.00E+00
EEE MJ 0.00E+00 0.00E+00 0.00E+00 0.00E+00 0.00E+00 0.00E+00 0.00E+00
ETE MJ 0.00E+00 0.00E+00 0.00E+00 0.00E+00 0.00E+00 0.00E+00 0.00E+00
CR Components for reuse; MR Materials for recycling; MER Materials for energy recovery; EEE Exported electric energy; ETE Exported thermal energy.
Information describing the biogenic carbon content at the factory gate
Biogenic carbon content Unit Value
Biogenic carbon content in product kg C 0.00
Biogenic carbon content in the accompanying packaging kg C 0.00
EPD for the best environmental decision 8
Additional requirements
Location based electricity mix from the use of electricity in manufacturing
National production mix from import, low voltage (production of transmission lines, in addition to direct
emissions and losses in grid) of applied electricity for the manufacturing prosess (foreground/core) per
functional unit.
GWP SUM
Foreground / core total
National electricity grid Data source [kg CO2 - [kg CO2 -
[kWh]
eq/kWh] eq]
market for electricity, low voltage | electricity, low Ecoinvent v3.9.1
0.40 0.0347 0.014
voltage | EN15804, NO (2023)
Guarantees of origin (GoO) from the use of electricity in the manufacturing phase
No electricity with GoO was used in the manufacturing phase.
Additional environmental impact indicators required for construction products
In order to increase the transparency of biogenic carbon contribution to climate impact, the indicator
GWP-IOBC is required as it declares climate impacts calculated according to the principle of
instantanious oxidation. GWP-IOBC is also reffered to as GWP-GHG in context to Swedish public
procurement legislation.
Parameter Unit A1-A3 A4 C1 C2 C3 C4 D
GWP-IOBC kg 5.32E+00 3.01E-02 6.21E-02 2.03E-03 7.79E-04 9.58E-05 -1.71E+00
GWP-IOBC Global warming potential calculated according to the principle of instantaneous oxidation.
Hazardous substances
The declaration is based upon reference to threshold values and/or test results and/or material safety
data sheets provided to EPD verifiers. Documentation available upon request to EPD owner.
☒ The product contains no substances given by the REACH Candidate list.
☐ The product contains substances given by the REACH Candidate list that are less than 0,1 % by
weight.
☐ The product contains dangerous substances, more then 0,1% by weight, given by the REACH
Candidate List, see table.
☐ The product contains no substances given by the REACH Candidate list.
☐ The product is classified as hazardous waste, see table.
Indoor environment
Not relevant to this product
Carbon footprint
Carbon footprint has not been worked out for the product.
EPD for the best environmental decision 9
Bibliography
ISO/TC 207/SC 3. (2006). ISO 14025:2006 Environmental labels and declarations — Type III environmental
declarations — Principles and procedures.
Acerinoc Europa, S.A.U. (2023). EPD - cold-rolled austenitic stainless steel.
ECO PLATFORM. (2023). ECO Platform Standards - General Remarks.
ECO PLATFORM. (2023, 12). LCA Calculation Rules and Specifications for EPDs.
EPD-Norge. (2021). NPCR 13 - Part B for steel and aluminium products (references to EN15804+A2).
ISO. (2006, 7 1). ISO 14025 Environmental labels and declarations - Type III environmental declarations -
Pricnicples and procedures. Geneva, Switzerland.
ISO. (2006). ISO 14044:2006 Environmental management — Life cycle assessment — Requirements and
guidelines. ISO/TC 207/SC 5.
ISO/TC 207. (2006). ISO 14040:2006(en) Environmental management — Life cycle assessment — Principles and
framework.
NS-EN. (2021). NS-EN 15804:2012+A2:2019+AC:2021: Sustainability of construction works - Environmental
product declarations - Core rules for the product category of construction products. NS-EN.
Spindler, C., & Ciroth, A. (2023, 6 19). EN 15804 add-on for ecoinvent by GreenDelta. Berlin, Germany.
The Norwegian EPD Foundation/EPD-Norge. (2023, 5 25). General Program Instructions 2019. Version 3.0.
Oslo, Norway. Retrieved from https://www.epd-norge.no/lover-og-regler/retningslinjer/
Program Operator tlf +47 23 08 80 00
The Norwegian EPD
Foundation
Post Box 5250 Majorstuen, 0303 e-
post@epd-norge.no
Oslo post:
Norway web www.epd-norge.no
Publisher tlf +47 23 08 80 00
The Norwegian EPD
Foundation
Post Box 5250 Majorstuen, 0303 e-
post@epd-norge.no
Oslo post:
Norway web www.epd-norge.no
Owner of the declaration tlf +47 51 78 81 00
Øglænd System AS Fax -
Engelsvollvegen 264 e-
oglaend@oglaend-system.com
4353 KLEPP STASJON post:
https://www.oglaend-
Norway web
system.no/kontakt/norge/
Author of the life cycle
tlf +47 98 25 90 10
assesment
Energiråd AS Fax -
e-
Trippevegen 1, 6009 Ålesund harald@energirad.no
post:
Norway web www.energirad.no
ECO Platform web www.eco-platform.org
ECO Portal web ECO Portal
EPD for the best environmental decision 10
