Environmental Product
Declaration
In accordance with ISO 14025 and EN 15804 +A2
Owner of the declaration: Q-bic plus infiltration
Norsk Wavin AS
system 100 m3
Program holder and publisher:
The Norwegian EPD foundation
Q-Bic Plus is a solution for
Declaration number: urban areas regarding
NEPD-3473-2071-EN stormwater management.
The Q-Bic Plus geocellular
Registration Number:
system has been uniquely
NEPD-3473-2071-EN
engineered to combine ease
Issue date: 27.05.2022 of access and speed of
The Norwegian EPD Foundation Valid to: 27.05.2027 installation.
Ver2-101122 Manufacturer
Wavin Netherlands B.V.
General information
Product:
Owner of the declaration:
Q-bic plus infiltration system 100 m3
Norsk Wavin AS
Contact person: Matteo Tagliaferri
Program Operator:
Phone: +31 623193684
The Norwegian EPD Foundation
e-mail: matteo.tagliaferri@wavin.com
Post Box 5250 Majorstuen, 0303 Oslo, Norway
Tlf: +47 23 08 80 00
Manufacturer:
e-mail: post@epd-norge.no
Wavin Netherlands B.V.
J.C. Kellerlaan 3, 7772 SG, Hardenberg,
Declaration number:
Netherlands
NEPD-3473-2071-EN Phone: +31 (0) 523 288165
e-mail: info@wavin.nl
This declaration is based on Product
Category Rules: Place of production:
CEN standard EN 15804:2012+A2:2019 serves as J.C. Kellerlaan 3, 7772 SG, Hardenberg,
core PCR, supplied with NPCR Part A, Version 2.0. Netherlands
Statements: Management system:
The owner of the declaration shall be liable for the EN ISO 9001:2015 and EN ISO 14001:2015
underlying information and evidence. EPD
Norway shall not be liable with respect to
Organisation no:
manufacturer, life cycle assessment data and
823355092
evidences.
Issue date:
Declared unit:
27.05.2022
100 m3 Q-bic plus infiltration system
Valid to:
Declared unit with option:
27.05.2027
A1,A2,A3,A4,A5,C1,C2,C3,C4,D
Year of study:
Functional unit:
2020
Not applicable.
Verification: Comparability:
Independent verification of the declaration and EPDs from other programmes than the Norwegian
data, according to ISO14025:2010 EPD foundation may not be comparable.
internal external
The EPD has been worked out by:
Lisa Overmars and Emma Thunnissen,
Ecochain Technologies
Harry van Ewijk, SGS Search
Independent verifier approved by EPD Norway
Approved (Manager of EPD Norway)
EPD for the best environmental decision 2
Product
Product description:
The Q-Bic Plus infiltration system is modular in its design and comprises of easy to install
components that can be designed to create a tank or soakaway to suit the needs of a specific
site. It is composed of:
- Column Unit
- Base Plate
- Side Plate
Product specification:
A typical composition of the Q-bic plus infiltration system, including packaging, is as follows:
Materials %
PP 99%
Additives 1%
Packaging 0%
The characteristics of the individual components the Q-bic plus infiltration system is composed
of are:
Characteristic components Q-bic plus infiltration system Value
Dimensions per column unit (nominal) (L x W x H) (mm) 1200 x 600 x 600
Gross volume per column unit (m3) 0.432
Net volume per column cell (m3) 0.417
Porosity (void ratio) (%) 95
Weight Column Unit (kg) 14,1
Weight Side Plate (kg) 2,8
Weight Base Plate (kg) 3,6
Technical data:
For this EPD, a double-layered Q-bic plus infiltration system of 100 m3 is considered. The
specifications of this system are:
Characteristic 100 m3 Q-bic plus infiltration system Value
Total weight system (kg) 4017
Column units (pieces) 242
Base plates (pieces) 120
Side plates (pieces) 61
Net volume (m3) 101,9
EPD for the best environmental decision 3
Gros volume (m3) 106,3
Tank surface area (m2) 218,6
Surface area of bottom (m2) 86,4
Surface area of sides (m2) 45,8
Actual installation depth (m) 2,23
Excavation volume (m3) 353,6
Backfill volume (m3) 247,3
The figure below shows an imagination of an installed Q-bic plus infiltration system of 100 m3 .
Market:
Europe, but the EPD is specific for Nordic countries.
Reference service life, product:
50 years
Reference service life, building:
LCA: Calculation rules
Declared unit:
100 m3 Q-bic plus infiltration unit
Data quality:
For module A1, specific data for product compositions as provided by the manufacturer are
used. For module A2, transportation data of the raw materials used to the production site was
collected. For module A3, energy consumption and waste production data was collected for
production year 2020. The used background processes are derived from Ecoinvent 3.6.
Allocation:
EPD for the best environmental decision 4
Allocation was carried out in accordance with the povisions of the EN15804. All manufacturing
inputs (energy and auxiliary materials) at production site level are allocated to different
production processes, followed by allocation of the production processes to the products that
are produced using these processes through mass allocation. No secondary materials have been
used in the production process.
System boundary:
Modules A1-A5 and C1-D are included. The figure below shows a (simplified) process tree.
Cut-off criteria:
All relevant inputs and outputs - like emissions, energy and materials - have been taken into
account in this LCA. In accordance with EN15804, the total neglected input flows per module
does not exceed 5% of energy usage and mass.
EPD for the best environmental decision 5
LCA: Scenarios and additional technical information
The following information describe the scenarios in the different modules of the EPD.
Transport from production place to assembly/user (A4)
The transportation distance from Hardenberg to Oslo was considerd.
Capacity utilisation
Type Type of vehicle Distance KM Fuel/Energy consumption
(incl. return) %
Truck 50% Unspecified 938 0,027 l diesel/tkm
Boat 50% Ferry 163 0,0295 kg heavy fuel oil/tkm
Assembly (A5)
Product losses of 2% are considered. Installation is done manually, but the excavation of the
sand is assumed to take place with a hydraulic digger. The diesel consumption for the hydraulic
digger is calculated from the excavation volume (m3) and the diesel consumption per m3.
Unit Value
Material loss kg 80,3
Packaging waste kg 0,075
Diesel consumption kg 46,37
End of Life (C1, C3, C4)
At the end-of-life, the demolition is done manually. However, the excavation of the sand is
assumed to take place with a hydraulic digger. The diesel consumption for the hydraulic digger
is calculated from the excavation volume (m3) and the diesel consumption per m3. The
considered waste treatment of the Q-bic plus infiltration unit components (PP column unit, base
plate and side plates) is 70% recycling, 20% incineration with energy recovery and 10%
landfill.
Unit Value
Diesel consumption kg 46,37
Collected as mixed construction waste kg 4017,4
Reuse kg 0
Recycling kg 2812,2
Energy recovery kg 803,5
To landfill kg 401,7
Transport to waste processing (C2)
The considered distances are 50 km to landfill, 100 km for energy recovery, and 250 km for
recycling.
Capacity utilisation
Type Type of vehicle Distance KM Fuel/Energy consumption
(incl. return) %
EPD for the best environmental decision 6
Truck 50% Unspecified 199,4 0,027 l diesel/tkm
Benefits and loads beyond the system boundaries (D)
For the PP and addives, 0,67 kg of saved virgin PP was considered per kg material recycled
(total of A5 en C3). The benefits from exported energy were calculation from the energy
efficiencies for Nothern countries reported by CEWEP, which is equal to an electrical efficiency
of 11,0%, and a thermal efficiency of 72,6%. Energy recovery from all materials (including
packaging) was considered. Substition of Norwegian electricity mix and district heating mix was
assumed.
Unit Value
Saving of virgin PP kg 1921,9
Substition of electric energy MJ 2930
Subsitition of thermal energy MJ 19340
Additional technical information
Not applicable
LCA: Results
The LCA results are presented below for the declared unit defined on page 2 of the EPD
document.
System boundaries (X=included, MND= module not declared, MNR=module not
relevant)
Benefits
& loads
Assembly
Product stage Use stage End of life stage beyond
stage
system
boundary
n -
s la ir e wt a am R t r o p s n a r T g n ir u t c a fu n a M t r o p s n a r T y lb m e s s A e s U e c n a n e t n ia M r ia p e R t n e m e c a lp e R t n e m h s ib r u fe R la n o ity ag rr eee pns Ou e la n o it ar re ete a ps w Ou n o io t cit ui rlo t sm ne od
c
-
t r o p s n a r T g n is s ee tc so ar Wp la s o p s iD g yn r eil v ec soy uc ce e RR --la it n e t o p
e e
D R
A1 A2 A3 A4 A5 B1 B2 B3 B4 B5 B6 B7 C1 C2 C3 C4 D
X X X X X X X X X X
Core environmental impact indicators
Indicator Unit A1-A3 A4 A5 C1 C2 C3 C4 D
GWP-total kg CO2 eq. 9,44E+03 5,68E+02 4,53E+02 1,89E+02 9,47E+01 3,07E+03 4,98E+01 -5,48E+03
GWP-fossil kg CO2 eq. 9,36E+03 5,68E+02 4,52E+02 1,89E+02 9,46E+01 3,07E+03 4,99E+01 -5,46E+03
EPD for the best e nvironmental decision 7
GWP-biogenic kg CO2 eq. 4,92E+01 2,85E-01 9,79E-01 7,25E-02 5,74E-02 -4,24E+00 4,34E-02 -1,77E+01
GWP-LULUC kg CO2 eq. 3,24E+01 2,20E-01 6,84E-01 1,97E-02 3,35E-02 5,94E-01 8,49E-04 -9,85E-01
ODP kg CFC11 eq. 3,39E-04 1,29E-04 5,09E-05 3,96E-05 2,18E-05 7,71E-05 1,25E-06 -2,72E-04
AP mol H⁺ eq. 3,57E+01 5,18E+00 2,82E+00 1,93E+00 5,39E-01 3,24E+00 2,98E-02 -1,45E+01
EP-freshwater kg P eq. 1,38E-01 4,36E-03 4,25E-03 1,04E-03 7,78E-04 1,71E-02 3,89E-05 -5,57E-02
EP-marine kg N eq. 6,54E+00 1,60E+00 1,03E+00 8,42E-01 1,93E-01 9,42E-01 1,94E-02 -2,59E+00
EP-terrestial mol N eq. 7,30E+01 1,77E+01 1,13E+01 9,24E+00 2,12E+00 1,04E+01 1,21E-01 -2,86E+01
kg NMVOC
POCP 3,05E+01 4,87E+00 3,34E+00 2,55E+00 6,07E-01 3,28E+00 4,54E-02 -1,31E+01
eq.
ADP-M&M kg Sb eq. 1,26E-01 1,33E-02 3,41E-03 3,26E-04 2,45E-03 1,29E-02 3,01E-05 -3,33E-02
ADP-fossil MJ 3,12E+05 8,53E+03 9,24E+03 2,58E+03 1,45E+03 1,03E+04 9,13E+01 -1,65E+05
WDP m³ 8,26E+03 2,46E+01 1,74E+02 4,53E+00 4,46E+00 2,02E+02 4,65E-01 -2,75E+03
GWP-total: Global Warming Potential; GWP-fossil: Global Warming Potential fossil fuels; GWP-biogenic:
Global Warming Potential biogenic; GWP-LULUC: Global Warming Potential land use and land use change;
ODP: Depletion potential of the stratospheric ozone layer; AP: Acidification potential, Accumulated
Exceedance; EP-freshwater: Eutrophication potential, fraction of nutrients reaching freshwater end
compartment; See “additional Norwegian requirements” for indicator given as PO4 eq. EP-marine:
Eutrophication potential, fraction of nutrients reaching freshwater end compartment; EP-terrestial:
Eutrophication potential, Accumulated Exceedance; POCP: Formation potential of tropospheric ozone; ADP-
M&M: Abiotic depletion potential for non-fossil resources (minerals and metals); ADP-fossil: Abiotic
depletion potential for fossil resources; WDP: Water deprivation potential, deprivation weighted water
counsumption
Additional environmental impact indicators
Indicator Unit A1-A3 A4 A5 C1 C2 C3 C4 D
Disease
PM 3,33E-04 4,69E-05 5,95E-05 5,07E-05 8,54E-06 5,34E-05 6,28E-07 -1,19E-04
incidence
kBq U235
IRP 2,54E+02 3,72E+01 1,75E+01 1,10E+01 6,35E+00 3,10E+01 4,23E-01 -7,76E+01
eq.
ETP-fw CTUe 7,44E+04 6,76E+03 3,59E+03 1,71E+03 1,18E+03 1,16E+04 7,64E+01 -1,94E+04
HTP-c CTUh 2,48E-06 2,58E-07 1,73E-07 8,88E-08 4,20E-08 1,40E-06 2,23E-09 -8,75E-07
HTP-nc CTUh 7,11E-05 7,82E-06 3,62E-06 1,67E-06 1,41E-06 1,73E-05 4,92E-08 -2,40E-05
Dimensionle
SQP 1,87E+04 6,64E+03 1,04E+03 3,41E+02 1,24E+03 8,23E+03 2,34E+02 -4,05E+03
ss
PM: Particulate matter emissions; IRP: Ionising radiation, human health; ETP-fw: Ecotoxicity (freshwater);
ETP-c: Human toxicity, cancer effects; HTP-nc: Human toxicity, non-cancer effects; SQP: Land use related
impacts / soil quality
Classification of disclaimers to the declaration of core and additional environmental
impact indicators
ILCD
Indicator Disclaimer
classification
Global warming potential (GWP) None
ILCD type / level
Depletion potential of the stratospheric ozone layer (ODP) None
1
Potential incidence of disease due to PM emissions (PM) None
Acidification potential, Accumulated Exceedance (AP) None
EPD for the best environmental decision 8
Eutrophication potential, Fraction of nutrients reaching freshwater end
None
compartment (EP-freshwater)
Eutrophication potential, Fraction of nutrients reaching marine end
None
compartment (EP-marine)
ILCD type / level
Eutrophication potential, Accumulated Exceedance (EP-terrestrial) None
2
Formation potential of tropospheric ozone (POCP) None
Potential Human exposure efficiency relative to U235 (IRP) 1
Abiotic depletion potential for non-fossil resources (ADP-minerals&metals) 2
Abiotic depletion potential for fossil resources (ADP-fossil) 2
Water (user) deprivation potential, deprivation-weighted water consumption
(WDP)
2
ILCD type / level
Potential Comparative Toxic Unit for ecosystems (ETP-fw) 2
3
Potential Comparative Toxic Unit for humans (HTP-c) 2
Potential Comparative Toxic Unit for humans (HTP-nc) 2
Potential Soil quality index (SQP) 2
Disclaimer 1 – This impact category deals mainly with the eventual impact of low dose ionizing radiation on
human health of the nuclear fuel cycle. It does not consider effects due to
possible nuclear accidents, occupational exposure nor due to radioactive waste disposal in underground facilities.
Potential ionizing radiation from the soil, from radon and from some
construction materials is also not measured by this indicator.
Disclaimer 2 – The results of this environmental impact indicator shall be used with care as the uncertainties on
these results are high or as there is limited experienced with the indicator
Resource use
Parameter Unit A1-A3 A4 A5 C1 C2 C3 C4 D
RPEE MJ 2,20E+04 1,15E+02 4,74E+02 2,06E+01 2,08E+01 5,08E+02 3,53E+00 -1,99E+03
RPEM MJ 0,00E+00 0,00E+00 0,00E+00 0,00E+00 0,00E+00 0,00E+00 0,00E+00 0,00E+00
TPE MJ 2,20E+04 1,15E+02 4,74E+02 2,06E+01 2,08E+01 5,08E+02 3,53E+00 -1,99E+03
NRPE MJ 3,34E+05 9,06E+03 9,87E+03 2,74E+03 1,54E+03 1,10E+04 9,69E+01 -1,78E+05
NRPM MJ 0,00E+00 0,00E+00 0,00E+00 0,00E+00 0,00E+00 0,00E+00 0,00E+00 0,00E+00
TRPE MJ 3,34E+05 9,06E+03 9,87E+03 2,74E+03 1,54E+03 1,10E+04 9,69E+01 -1,78E+05
SM kg 0,00E+00 0,00E+00 0,00E+00 0,00E+00 0,00E+00 0,00E+00 0,00E+00 0,00E+00
RSF MJ 0,00E+00 0,00E+00 0,00E+00 0,00E+00 0,00E+00 0,00E+00 0,00E+00 0,00E+00
NRSF MJ 0,00E+00 0,00E+00 0,00E+00 0,00E+00 0,00E+00 0,00E+00 0,00E+00 0,00E+00
W m3 1,53E+02 9,06E-01 3,37E+00 1,60E-01 1,64E-01 5,94E+00 1,13E-01 -4,07E+01
RPEE Renewable primary energy resources used as energy carrier; RPEM Renewable primary energy
resources used as raw materials; TPE Total use of renewable primary energy resources; NRPE Non
renewable primary energy resources used as energy carrier; NRPM Non renewable primary energy
resources used as materials; TRPE Total use of non renewable primary energy resources; SM Use of
secondary materials; RSF Use of renewable secondary fuels; NRSF Use of non renewable secondary fuels; W
Use of net fresh water
End of life - Waste
Parameter Unit A1-A3 A4 A5 C1 C2 C3 C4 D
EPD for the best environmental decision 9
HW KG 7,71E-02 2,03E-02 9,48E-03 7,12E-03 3,71E-03 1,67E-02 1,10E-04 -4,58E-02
NHW KG 6,97E+02 4,74E+02 4,81E+01 4,70E+00 9,00E+01 5,05E+02 4,02E+02 -1,24E+02
RW KG 2,87E-01 5,82E-02 2,54E-02 1,75E-02 9,88E-03 3,93E-02 5,96E-04 -7,23E-02
HW Hazardous waste disposed; NHW Non hazardous waste disposed; RW Radioactive waste disposed
End of life – output flow
Parameter Unit A1-A3 A4 A5 C1 C2 C3 C4 D
CR kg 0,00E+00 0,00E+00 0,00E+00 0,00E+00 0,00E+00 0,00E+00 0,00E+00 0,00E+00
MR kg 0,00E+00 0,00E+00 5,62E+01 0,00E+00 0,00E+00 2,81E+03 0,00E+00 0,00E+00
MER kg 0,00E+00 0,00E+00 1,61E+01 0,00E+00 0,00E+00 8,03E+02 0,00E+00 0,00E+00
EEE MJ 0,00E+00 0,00E+00 0,00E+00 0,00E+00 0,00E+00 0,00E+00 0,00E+00 2,93E+03
ETE MJ 0,00E+00 0,00E+00 0,00E+00 0,00E+00 0,00E+00 0,00E+00 0,00E+00 1,93E+04
CR Components for reuse; MR Materials for recycling; MER Mater ials for energy recovery; EEE Exported
electric energy; ETE Exported thermal energy
Information describing the biogenic carbon content at the factory gate
Biogenic carbon content Unit Value
Biogenic carbon content in product kg C 0
Biogenic carbon content in the accompanying packaging kg C 0
Additional Norwegian requirements
Greenhous gas emission from the use of electricity in the manufacturing phase
National production mix from import, low voltage (production of transmission lines, in addition
to direct emissions and losses in grid) of applied electricity for the manufacturing process(A3).
National electricity grid Unit Value
94% Hydroelectricity, average & 6% solar electricity (Ecoinvent 3.6) kg CO2 -eq/kWh 0,0528
Additional environmental impact indicators required in NPCR Part A for construction
products
In order to increase the transparency of biogenic carbon contribution to climate impact, the
indicator for GWP has been sub-divided into the following:
GWP-IOBC Climate impacts calculated according to the principle of instantaneous
oxidationGWP-BC Climate impacts from the net uptake and emission of biogenic carbon
from each module.
Indicator Unit A1-A3 A4 A5 C1 C2 C3 C4 D
GWP-IOBC kg CO2 eq. 9,39E+03 5,68E+02 4,52E+02 1,89E+02 9,46E+01 3,07E+03 4,98E+01 -5,46E+03
GWP-BC kg CO2 eq. 4,92E+01 2,85E-01 9,79E-01 7,25E-02 5,74E-02 -4,24E+00 4,34E-02 -1,77E+01
EPD for the best environmental decision 10
GWP kg CO2 eq. 9,44E+03 5,68E+02 4,53E+02 1,89E+02 9,47E+01 3,07E+03 4,98E+01 -5,48E+03
EP-freshwater* Eutrophication potential, fraction of nutrients reaching freshwater end compartment.
Declared as PO4 eq. GWP-IOBC Global warming potential calculated according to the principle of
instantanious oxidation. GWP-BC Global warming potential from net uptake and emissions of biogenic
carbon from the materials in each module. GWP Global warming potential
Hazardous substances
The declaration is based upon reference to threshold values and/or test results and/or material
safety data sheets provided to EPD verifiers. Documentation available upon request to EPD
owner.
✓ The product contains no substances given by the REACH Candidate list or the
Norwegian priority list.
□ The product contains substances given by the REACH Candidate list or the Norwegian
priority list that are less than 0,1 % by weight.
□ The product contain dangerous substances, more then 0,1% by weight, given by the
REACH Candidate List or the Norwegian Priority list, see table.
□ The product contains no substances given by the REACH Candidate list or the
Norwegian priority list. The product is classified as hazardous waste (Avfallsforskiften,
Annex III), see table.
Indoor environment
The product meets the requirements for low emissions.
Carbon footprint
Carbon footprint has not been worked out for the product.
EPD for the best environmental decision 11
Bibliography
ISO 14025:2010 Environmental labels and declarations - Type III environmental
declarations - Principles and procedures
ISO 14044:2006 Environmental management - Life cycle assessment -
Requirements and guidelines
EN 15804:2012+A2:2019 Sustainability of construction works - Environmental product
declaration - Core rules for the product category of construction
products
ISO 21930:2007 Sustainability in building construction - Environmental
declaration of building products
NPCR Part A Construction products and services. Ver. 2.0. March 2021, EPD-
Norge
CEWEP Results of Specific Data for Energy, R1 Plant Efficiency Factor and
NCV of 314 European Waste-to-Energy (WtE) Plants, CEWEP
Energy Report III (status 2007-2010), 2012, Reiman, D.O.
Program Operator tlf +47 23 08 80 00
The Norwegian EPD Foundation
Post Box 5250 Majorstuen, 0303 Oslo e-post: post@epd-norge.no
Norway web www.epd-norge.no
Publisher tlf +47 23 08 80 00
The Norwegian EPD Foundation
Post Box 5250 Majorstuen, 0303 Oslo e-post: post@epd-norge.no
Norway web www.epd-norge.no
Owner of the declaration tlf +4745190625
Norsk Wavin AS Fax
Karihaugveien 89, 1086, Oslo e-post: Invoice.no@wavin.com
Norway web www.wavin.com/nn-no
Author of the life cycle assessment tlf +31 (0)20 303 5777
Lisa Overmars Fax
H.J.E. Wenckebachweg 123, 1096 AM
e-post: lovermars@ecochain.com
Amsterdam
The Netherlands web www.ecochain.com
EPD for the best environmental decision 12
EPD for the best
environmental
decision
The Norwegian EPD foundation
www.epd-norge.no
