Environmental product declaration
in accordance with ISO 14025 and EN 15804+A2
12kV , 31.5 kA , SBB Air Insulated Switchgear : Feeder and Transformer Type - AH12
Owner of the declaration: Program operator:
Al-Ahleia Switchgear Co., k.s.c.c The Norwegian EPD Foundation
Product: Declaration number:
12kV , 31.5 kA , SBB Air Insulated Switchgear : Feeder
and Transformer Type - AH12 NEPD-8817-8477
Declared unit: Registration number:
1 pcs
NEPD-8817-8477
This declaration is based on Product Category Rules:
Issue date: 23.01.2025
CEN Standard EN 15804:2012+A2:2019, EN 50693:2019
The Norwegian EPD Foundation and PCR EPD Italy 007 serves as core PCR Valid to: 23.01.2030
PCR EPDItaly015 - Electronic and electrical products and
systems - Switchboards EPD software:
LCAno EPD generator ID: 507936
1 / 14
General information
Product Owner of the declaration:
12kV , 31.5 kA , SBB Air Insulated Switchgear : Feeder and Al-Ahleia Switchgear Co., k.s.c.c
Transformer Type - AH12 Contact person: Manoj C.G
Phone: +965 24271000
e-mail: ahleia@ahleiasg.com
Program operator: Manufacturer:
The Norwegian EPD Foundation Al-Ahleia Switchgear Co., k.s.c.c
Post Box 5250 Majorstuen, 0303 Oslo, Norway
Phone: +47 977 22 020
web: www.epd-norge.no
Declaration number: Place of production:
Al-Ahleia Switchgear Co., k.s.c.c
NEPD-8817-8477
, Kuwait
This declaration is based on Product Category Rules: Management system:
CEN Standard EN 15804:2012+A2:2019, EN 50693:2019 and PCR ISO 9001, 14001, 29001 and 45001
EPD Italy 007 serves as core PCR
PCR EPDItaly015 - Electronic and electrical products and systems -
Switchboards
Statement of liability: Organisation no:
The owner of the declaration shall be liable for the underlying 33118
information and evidence. EPD Norway shall not be liable with respect
to manufacturer information, life cycle assessment data and
evidences.​
Declared unit: Issue date:
1 pcs 12kV , 31.5 kA , SBB Air Insulated Switchgear : Feeder and
23.01.2025
Transformer Type - AH12
Declared unit with option: Valid to:
A1-A3,A4,A5,B6,C1,C2,C3,C4,D 23.01.2030
Year of study:
2023
Functional unit: Comparability:
Functional unit - 1 SBB Switchgear : Feeder and Transformer type - EPD for electronic and electrical products and systems may not be
AH12 12kV , 31.5 kA , with a use rate of 99% and average load factor comparable if they do not comply with similar PCR standards.
of 55.5 % (an assembly of electric and electronic devices delivering
control, distribution and safety functions) manufactured and installed,
used over a lifetime of 20 years, including waste treatment at end-of-
life.
General information on verification of EPD from EPD tools: Development and verification of EPD:
Independent verification of data, other environmental information The declaration is created using EPD tool lca.tools ver EPD2022.03,
and the declaration according to EN ISO 14025:2010, § 8.1.3 and § developed by LCA.no. The EPD tool is integrated in the company's
8.1.4. Verification of each EPD is made according to EPD-Norway’s management system, and has been approved by EPD Norway.
guidelines for verification and approval requiring that tools are i)
integrated into the company's environmental management system, ii) Developer of EPD: Zohaib Ali
the procedures for use of the EPD tool are approved by EPD-Norway,
Reviewer of company-specific input data and EPD:​ Børge Heggen
and iii) the process is reviewed annually by an independent third
Johansen, Energiråd AS
party verifier. See Appendix G of EPD-Norway's General Programme
Instructions for further information on EPD tools
Verification of EPD tool: Approved:
2 / 14
Independent third party verification of the EPD tool, background data
and test-EPD in accordance with EPDNorway's procedures and
guidelines for verification and approval of EPD tools. Approval
number: NEPDT57.
Third party verifier:
Elisabet Amat, GREENIZE projects
(no signature required)
3 / 14
Product
Product description:
Al-Ahleia make SBB Air insulated switchgear Type: AH12 is an indoor, totally enclosed type metal clad switchgear equipped with a horizontal
isolation Switching Device. Type AH12 Switchgear fulfil the common need of controlling, protecting and isolating power systems. SBB Type: AH12
Switchgear is supplied in a number of different configurations and ratings suitable for switching application in 12/17.5kV Distribution Networks
such as in Utility Substations, Package Substations, Power plants, Refineries or Offshore Platforms.
The product with switching device a circuit breaker, described in this declaration will control either: (a) Feeder Circuit or (b) the Power Transformer
Circuit.
Product specification
Al- Ahleia Make SBB switchgear Type AH 12 is designed and manufactured to fully comply with the requirements specified in International
Standards and relevant Customer specifications.
Standard
IEC 62271-1 High Voltage Switchgear
IEC 62271-100 Alternating current circuit breakers
IEC 62271-200 Alternating-current metal-enclosed switchgear for rated voltages higher than 1 kV and less than or equal to 52 kV
IEC 62271-102 Alternating current disconnectors and earthing switches
IEC 60529 Degrees of protection provided by the enclosures (IP code)
Materials kg %
Electronic - Cable 3,99 0,55
Electronic - Relay 14,76 2,02
Electronic - Switch 0,36 0,05
Plastic - Polyvinyl chloride (PVC) 7,86 1,08
Powder coating 5,97 0,82
Electronics 1,05 0,14
Metal 644,50 88,15
Chemical 46,33 6,34
Others 0,67 0,09
Paper 1,71 0,23
Plastic - Polycarbonate (PC) 3,93 0,54
Total 731,13 100,00
Packaging kg %
Packaging - Plastic 0,75 1,23
Packaging - Wood 60,00 98,77
Total incl. packaging 791,88 100,00
Technical data:
Rated Voltage: 12/ 15 kV
Rated Insulation Level :28 /95 kVp
Rated Frequency: 50/60 Hz
Rated Short Time Withstand Current: 31.5 kA
Rated duration of Short -Circuit: 3 Sec
Rated Peak Withstand Current: 80 kA
Rated Current Feeder: 1000 A (IEC) / … 800 A (kuwait Ambient)
Internal Arc Classification: AFLR 31.5 KA – 1Sec.
Market:
Average distribution to middle east and gulf cooperation council countries (300 km).
Reference service life, product
20 Years
Reference service life, building or construction works
N/A
LCA: Calculation rules
Declared unit:
1 pcs 12kV , 31.5 kA , SBB Air Insulated Switchgear : Feeder and Transformer Type - AH12
Cut-off criteria:
All major raw materials and all the essential energy is included. The production processes for raw materials and energy flows with very small
amounts (less than 1%) are not included. These cut-off criteria do not apply for hazardous materials and substances.
4 / 14
Allocation:
The allocation is made in accordance with the provisions of EN 15804. Incoming energy and water and waste production in-house is allocated
equally among all products through mass allocation. Effects of primary production of recycled materials is allocated to the main product in which
the material was used. The recycling process and transportation of the material is allocated to this analysis.
Data quality:
Specific data for the product composition are provided by the manufacturer. The data represent the production of the declared product and were
collected for EPD development in the year of study. Background data is based on EPDs according to EN 15804 and different LCA databases. The
data quality of the raw materials in A1 is presented in the table below.
Materials Source Data quality Year
Supplier data +
Chemical ecoinvent 3.6 2019
database
Electronic - Cable Ecoinvent 3.6 Database 2019
Supplier data +
Electronic - Cable ecoinvent 3.6 2019
database
Electronic - Relay ecoinvent 3.6 Database 2019
Supplier data +
Electronic - Relay ecoinvent 3.6 2019
database
Supplier data +
Electronic - Switch ecoinvent 3.6 2019
database
Electronics ecoinvent 3.6 Database 2019
Supplier data +
Electronics ecoinvent 3.6 2019
database
Metal ecoinvent 3.6 Database 2019
Metal Modified ecoinvent 3.6 Database 2019
Others ecoinvent 3.6 Database 2019
Packaging - Plastic ecoinvent 3.6 Database 2019
Packaging - Wood ecoinvent 3.6 Database 2019
Paper ecoinvent 3.6 Database 2019
Plastic - Polycarbonate (PC) ecoinvent 3.6 Database 2019
Plastic - Polyvinyl chloride (PVC) ecoinvent 3.6 Database 2019
Powder coating Ecoinvent 3.6 Database 2019
5 / 14
System boundaries (X=included, MND=module not declared, MNR=module not relevant)
Construction Beyond the system
Product stage Use stage End of life stage
installation stage boundaries
A1 A2 A3 A4 A5 B1 B2 B3 B4 B5 B6 B7 C1 C2 C3 C4 D
X X X X X MND MND MND MND MND X MND X X X X X
System boundary:
Additional technical information:
The reference product 12kV , 31.5 kA , SBB Switchgear : Feeder Type - AH12 represents the product family based on the highest material
consumption. And SBB Switchgear : Transformer feeder type slightly changes due to its usage in Switching application of 12 kV/ 415 V power
transformer HV side . Transformer is protected by the non- directional over current and earth fault relays functioning in the Transformer feeder
units . Additionally transformer units are equipped with auxiliary trip relays to receive trip signals from connected transformer.
waR slairetam tropsnarT gnirutcafunaM tropsnarT ylbmessA e​sU ecnanetniaM riapeR tnemecalpeR tnemhsibrufeR lanoitarepO ygrene esu lanoitarepO esu retaw -eD noitcurtsnoc noitilomed tropsnarT etsaW gnissecorp lasopsiD -yrevoceR-esueR laitnetop-gnilcyceR
6 / 14
LCA: Scenarios and additional technical information
The following information describe the scenarios in the different modules of the EPD.
Module A4 = Average distribution to middle east and gulf cooperation council countries (300 km).
Module A5 = Installation is performed by manual labor, with the use of electrical machines, that fall under the cut-off criteria of 1% and is
therefore neglected. Packaging of the final product consist of wooden pallet and plastic packaging.
Module B6 = The operational energy use of the switchgear is calculated based on the methodology provided in EPD Italy PCR -015 for
switchboards. To calculate the electricity use of the switchgear, the following scenario parameters have been applied:
- Reference power consumption in Watts (Puse) = 340.55 watt
- Standard year time (ty) = 8760 hours
- Use Time rate (a) = 99.5%
- Euse [kWh] = 59366.0382
Module C1 = The de-installation of the switchgear is carried out manually, with the assistance of electrical tools. The energy consumption of
portable electrical devices (e.g., drills) is typically low, falling below the 1% cut-off criterion, and is therefore disregarded.
Module C2 = Transportation from building site to the waste treatment facility with an average distance of 300km.
Modules C3 and C4 = Waste treatment of the product follows the default values provided in EN 50693, Product Category Rules for life cycle
assessments of electronic and electrical products and systems, table G.4. This table specified how different types of raw materials used in A1 will
likely be treated during the end-of-life of the product. Waste treatments in C3 include material recycling and incineration with and without energy
recovery and fly ash extraction. Disposal in C4 consist of landfilling of different waste fractions and of ashes.
Module D = The recyclability of metals, plastics, and electronic components allows the producers a credit for the net scrap that is produced at the
end of a product’s life. The benefits from recycling of net scrap are described in formula from EN 15804:2012+A2:2019. Substitution of heat and
electricity generated by the incineration with energy recovery of plastic insulation and other parts is also calculated in module D.
Capacity utilisation Value
Transport from production place to user (A4) Distance (km) Fuel/Energy Consumption Unit
(incl. return) % (Liter/tonne)
Truck, 16-32 tonnes, EURO 6 (km) - Rest of World 38,8 % 300 0,044 l/tkm 13,20
Assembly (A5) Unit Value
Waste, wood, to average treatment - A5 including
kg 60,000000000
transport (kg)
Waste, packaging, plastic film (LDPE), to average
kg 0,75
treatment (kg)
Operational energy (B6) Unit Value
Electricity, medium voltage (kWh) - Middle East
kWh 59366,038
average
Capacity utilisation Value
Transport to waste processing (C2) Distance (km) Fuel/Energy Consumption Unit
(incl. return) % (Liter/tonne)
Truck, 16-32 tonnes, EURO 6 (km) - Rest of World 38,8 % 300 0,044 l/tkm 13,20
Waste processing (C3) Unit Value
Metal to recycling (kg) kg 500,76
Waste treatment of plastic mixture, incineration
kg 34,42
with energy recovery and fly ash extraction (kg)
Waste treatment per kg used electronic
kg 18,62
components, manual seperation (kg)
Waste, Metals to recycling (kg) kg 3,89
Waste treatment per kg electronics scrap from
PWB, without components, recycling of copper - kg 0,58
(kg)
Waste treatment per kg electronics scrap from
kg 0,29
PWB, with components, recycling of metals (kg)
Waste treatment per kg Non-hazardous waste,
kg 1,70
incineration with fly ash extraction - (kg)
Waste treatment per kg Emulsion Paint,
kg 5,96
hazardous waste incineration (kg)
7 / 14
Disposal (C4) Unit Value
Landfilling of Metal (kg) kg 148,033
Landfilling of ashes from incineration of Plastic
kg 1,20
mixture, process per kg ashes and residues (kg)
Landfilling of plastic mixture (kg) kg 34,42
Landfilling of hazardous waste (kg) kg 0,95
Landfilling of ashes from incineration of Non-
hazardous waste, process per kg ashes and kg 0,40
residues (kg)
Landfilling of ashes from incineration of Emulsion
Paint, hazardous waste incineration, process of kg 4,21
ashes and residues (kg)
Benefits and loads beyond the system
Unit Value
boundaries (D)
Substitution of primary steel with net scrap (kg) kg 242,85
Substitution of primary copper with net scrap (kg) kg 23,90
Substitution of primary Brass with net scrap (kg) kg 1,77
Substitution of primary aluminium with net scrap
kg 0,084
(kg)
Substitution of electricity (MJ) MJ 53,90
Substitution of thermal energy, district heating
MJ 815,52
(MJ)
Substitution of primary other ferrous metals with
kg 3,73
net scrap (kg)
Substitution of primary metals with net scrap
kg 0,081
from PWB, with components (kg)
8 / 14
LCA: Results
The LCA results are presented below for the declared unit defined on page 2 of the EPD document.
Environmental impact
Indicator Unit A1-A3 A4 A5 B6 C1 C2 C3 C4 D
GWP-total kg CO2 -eq 6,02E+03 4,08E+01 9,26E+01 5,03E+04 0 4,08E+01 1,01E+02 7,53E+00 -3,47E+02
GWP-fossil kg CO2 -eq 6,04E+03 4,07E+01 1,67E+00 5,03E+04 0 4,07E+01 1,00E+02 7,53E+00 -3,46E+02
GWP-biogenic kg CO2 -eq -2,97E+01 1,59E-02 9,10E+01 4,39E+00 0 1,59E-02 9,65E-01 1,10E-03 -4,84E-01
GWP-luluc kg CO2 -eq 3,89E+00 1,49E-02 4,19E-04 1,69E+00 0 1,49E-02 8,30E-03 2,84E-03 -3,78E-01
ODP kg CFC11 -eq 6,70E-04 8,86E-06 2,61E-07 8,15E-03 0 8,86E-06 2,04E-06 7,75E-07 -3,44E-01
AP mol H+ -eq 1,12E+02 1,22E-01 1,31E-02 3,71E+02 0 1,22E-01 5,32E-02 2,42E-02 -1,20E+01
EP-FreshWater kg P -eq 8,92E-01 3,82E-04 1,95E-05 7,69E-02 0 3,82E-04 2,47E-04 6,92E-05 -8,91E-02
EP-Marine kg N -eq 8,92E+00 2,40E-02 5,64E-03 5,29E+01 0 2,40E-02 1,47E-02 1,24E-02 -7,37E-01
EP-Terrestial mol N -eq 1,28E+02 2,68E-01 5,99E-02 5,81E+02 0 2,68E-01 1,57E-01 9,49E-02 -9,84E+00
POCP kg NMVOC -eq 3,30E+01 1,00E-01 1,54E-02 1,66E+02 0 1,00E-01 4,25E-02 2,75E-02 -3,26E+00
ADP-minerals&metals1 kg Sb-eq 1,73E+00 1,09E-03 2,65E-05 5,09E-02 0 1,09E-03 7,74E-05 2,27E-05 -1,11E-01
ADP-fossil1 MJ 7,54E+04 6,02E+02 1,92E+01 6,80E+05 0 6,02E+02 1,29E+02 6,59E+01 -3,02E+03
WDP1 m3 4,41E+04 1,96E+02 3,01E+01 2,48E+05 0 1,96E+02 5,57E+02 1,47E+03 1,57E+04
GWP-total = Global Warming Potential total; GWP-fossil = Global Warming Potential fossil fuels; GWP-biogenic = Global Warming Potential biogenic; GWP-luluc =
Global Warming Potential land use and land use change; ODP = Depletion potential of the stratospheric ozone layer; AP = Acidification potential, Accumulated
Exceedance; EP-freshwater = Eutrophication potential, fraction of nutrients reaching freshwater end compartment: EP-marine = Eutrophication potential, fraction of
nutrients reaching marine end compartment; EP-terrestrial = Eutrophication potential, Accumulated Exceedance; POCP = Formation potential of tropospheric ozone;
ADP-minerals&metals = Abiotic depletion potential for non-fossil resources; ADP-fossil = Abiotic depletion for fossil resources potential; WDP = Water (user)
deprivation potential, deprivation-weighted water consumption
"Reading example: 9,0 E-03 = 9,0*10-3 = 0,009"
*INA Indicator Not Assessed
1. The results of this environmental impact indicator shall be used with care as the uncertainties on these results are high or as there is limited experienced with the
indicator
Remarks to environmental impacts
9 / 14
Additional environmental impact indicators
Indicator Unit A1-A3 A4 A5 B6 C1 C2 C3 C4 D
PM Disease incidence 4,98E-04 2,63E-06 1,60E-07 2,68E-03 0 2,63E-06 5,56E-07 4,40E-07 -4,62E-05
IRP2 kgBq U235 -eq 2,12E+02 2,50E+00 6,99E-02 2,04E+03 0 2,50E+00 5,77E-01 4,05E-01 -7,22E-01
ETP-fw1 CTUe 7,35E+05 4,88E+02 2,18E+01 2,50E+05 0 4,88E+02 4,79E+02 9,17E+04 -1,13E+05
HTP-c1 CTUh 2,64E-05 0,00E+00 2,41E-09 1,50E-05 0 0,00E+00 1,43E-08 7,07E-09 -2,67E-06
HTP-nc1 CTUh 1,25E-03 4,79E-07 1,16E-07 1,47E-04 0 4,79E-07 7,24E-07 1,31E-07 -8,77E-05
SQP1 dimensionless 3,17E+04 4,12E+02 1,11E+01 6,71E+04 0 4,12E+02 4,82E+01 1,37E+02 -1,87E+03
PM = Particulate Matter emissions; IRP = Ionizing radiation – human health; ETP-fw = Eco toxicity – freshwater; HTP-c = Human toxicity – cancer effects; HTP-nc =
Human toxicity – non cancer effects; SQP = Potential Soil Quality Index (dimensionless)
"Reading example: 9,0 E-03 = 9,0*10-3 = 0,009"
*INA Indicator Not Assessed
1. The results of this environmental impact indicator shall be used with care as the uncertainties on these results are high or as there is limited experienced with the
indicator
2. This impact category deals mainly with the eventual impact of low dose ionizing radiation on human health of the nuclear fuel cycle. It does not consider effects due
to possible nuclear accidents, occupational exposure nor due to radioactive waste disposal in underground facilities. Potential ionizing radiation from the soil, from
radon and from some construction materials is also not measured by this indicator.
10 / 14
Resource use
Indicator Unit A1-A3 A4 A5 B6 C1 C2 C3 C4 D
PERE MJ 4,63E+03 6,81E+00 3,96E-01 2,13E+03 0 6,81E+00 2,19E+01 8,70E+00 -8,39E+02
PERM MJ 8,40E+02 0,00E+00 -8,33E+02 0,00E+00 0 0,00E+00 -7,40E+00 0,00E+00 0,00E+00
PERT MJ 5,47E+03 6,81E+00 -8,32E+02 2,13E+03 0 6,81E+00 1,45E+01 8,70E+00 -8,39E+02
PENRE MJ 7,49E+04 6,02E+02 1,92E+01 6,80E+05 0 6,02E+02 1,29E+02 6,59E+01 -3,02E+03
PENRM MJ 1,12E+03 0,00E+00 -3,19E+01 0,00E+00 0 0,00E+00 -1,07E+03 0,00E+00 0,00E+00
PENRT MJ 7,60E+04 6,02E+02 -1,26E+01 6,80E+05 0 6,02E+02 -9,46E+02 6,59E+01 -3,02E+03
SM kg 2,82E+02 0,00E+00 0,00E+00 0,00E+00 0 0,00E+00 0,00E+00 2,06E-02 1,61E+01
RSF MJ 4,43E+01 1,33E-01 1,15E-02 3,91E+01 0 1,33E-01 4,73E-01 1,68E-01 1,11E+01
NRSF MJ 1,04E+03 1,13E+00 1,30E-01 2,00E+02 0 1,13E+00 -2,10E-04 3,03E-01 2,64E+02
FW m3 4,51E+01 6,73E-02 1,39E-02 1,16E+02 0 6,73E-02 1,49E-01 8,52E-02 -2,71E+00
PERE = Use of renewable primary energy excluding renewable primary energy resources used as raw materials; PERM = Use of renewable primary energy resources used
as raw materials; PERT = Total use of renewable primary energy resources; PENRE = Use of non renewable primary energy excluding non-renewable primary energy
resources used as raw materials; PENRM = Use of non renewable primary energy resources used as raw materials; PENRT = Total use of non renewable primary energy
resources; SM = Use of secondary materials; RSF = Use of renewable secondary fuels; NRSF = Use of non-renewable secondary fuels; FW = Net use of fresh water
"Reading example: 9,0 E-03 = 9,0*10-3 = 0,009"
*INA Indicator Not Assessed
11 / 14
End of life - Waste
Indicator Unit A1-A3 A4 A5 B6 C1 C2 C3 C4 D
HWD kg 3,47E+01 5,44E-02 0,00E+00 6,08E+01 0 5,44E-02 1,73E-04 6,88E+00 -2,15E+00
NHWD kg 9,97E+02 2,89E+01 6,08E+01 7,15E+02 0 2,89E+01 1,97E+00 1,89E+02 -1,44E+02
RWD kg 2,75E-01 3,95E-03 0,00E+00 3,31E+00 0 3,95E-03 9,92E-06 3,96E-04 -7,12E-04
HWD = Hazardous waste disposed; NHWD = Non-hazardous waste disposed; RWD = Radioactive waste disposed
"Reading example: 9,0 E-03 = 9,0*10-3 = 0,009"
*INA Indicator Not Assessed
End of life - Output flow
Indicator Unit A1-A3 A4 A5 B6 C1 C2 C3 C4 D
CRU kg 0,00E+00 0,00E+00 0,00E+00 0,00E+00 0 0,00E+00 0,00E+00 0,00E+00 0,00E+00
MFR kg 1,98E+02 0,00E+00 3,84E-01 0,00E+00 0 0,00E+00 5,05E+02 3,09E-03 -7,32E-01
MER kg 2,82E+01 0,00E+00 6,00E+01 0,00E+00 0 0,00E+00 4,21E+01 7,55E-05 -9,55E-02
EEE MJ 1,66E+01 0,00E+00 4,17E+01 0,00E+00 0 0,00E+00 5,29E+01 4,90E-03 -2,70E-01
EET MJ 2,50E+02 0,00E+00 6,31E+02 0,00E+00 0 0,00E+00 8,00E+02 7,41E-02 -4,09E+00
CRU = Components for re-use; MFR = Materials for recycling; MER = Materials for energy recovery; EEE = Exported energy electrical; EET = Exported energy thermal
"Reading example: 9,0 E-03 = 9,0*10-3 = 0,009"
*INA Indicator Not Assessed
Biogenic Carbon Content
Indicator Unit At the factory gate
Biogenic carbon content in product kg C 2,44E-01
Biogenic carbon content in accompanying packaging kg C 2,48E+01
Note: 1 kg biogenic carbon is equivalent to 44/12 kg CO2
12 / 14
Additional requirements
Greenhouse gas emissions from the use of electricity in the manufacturing phase
National production mix from import, low voltage (production of transmission lines, in addition to direct emissions and losses in grid) of applied
electricity for the manufacturing process (A3).
Electricity mix Source Amount Unit
Electricity, low voltage (kWh) - Kuwait ecoinvent 3.6 938,36 g CO2-eq/kWh
Dangerous substances
The product contains no substances given by the REACH Candidate list.
Indoor environment
Additional Environmental Information
Additional environmental impact indicators required in NPCR Part A for construction products
Indicator Unit A1-A3 A4 A5 B6 C1 C2 C3 C4 D
GWPIOBC kg CO2 -eq 6,10E+03 4,08E+01 1,67E+00 5,03E+04 0 4,08E+01 9,84E+01 8,06E+00 -4,51E+02
GWP-IOBC: Global warming potential calculated according to the principle of instantaneous oxidation. In order to increase the transparency of biogenic carbon​
contribution to climate impact, the indicator GWP-IOBC is required as it declares climate impacts calculated according to the principle of instantaneous oxidation.​
GWP-IOBC is also referred to as GWP-GHG in context to Swedish public procurement legislation.
13 / 14
Bibliography
EN ISO 14025:2010. Environmental labels and declarations - Type III environmental declarations - Principles and procedures. International
Organization for Standardization.
ISO 14044:2006. Environmental management - Life cycle assessment - Requirements and guidelines. International Organization for
Standardization.
EN 15804:2012+A2:2019. Environmental product declaration - Core rules for the product category of construction products. European
Committee for Standardization.
ISO 21930:2017. Sustainability in buildings and civil engineering works - Core rules for environmental product declarations of construction
products. International Organization for Standardization.
EN 50693:2019. Product category rules for life cycle assessments of electronic and electrical products and systems. European Committee for
Standardization.
Ecoinvent v3, 2019. Allocation, cut-off by classification. Swiss Centre of Life Cycle Inventories.
Iversen et al., (2021). eEPD v2021.09, background information for EPD generator tool system verification, LCA.no. Report number: 07.21. System
verification report.
Ali & Graafland (2024). EPD generator for PCR EPD Italy 015 part B for switchboards, background information for EPD generator application and
LCA data, LCA.no. Report number: 14.24. PCR verification report.
EPD Italy (2020). PCR EPD Italy 007 Part A for electronic and electrical products and systems. EPD Italy. Version 3, issue 13-01-2023 and valid
until 19-01-2025.
EPD Italy (2020). PCR EPD Italy 015 Part B for switcboards. EPD Italy. Version 0, issue 23-02-2022 and valid until 24-09-2025.
Program operator and publisher Phone: +47 977 22 020
The Norwegian EPD Foundation e-mail: post@epd-norge.no
Post Box 5250 Majorstuen, 0303 Oslo, Norway web: www.epd-norge.no
Owner of the declaration: Phone: +965 24271000
Al-Ahleia Switchgear Co., k.s.c.c e-mail: ahleia@ahleiasg.com
, , Kuwait web: https://www.ahleiasg.com
Author of the Life Cycle Assessment Phone: +47 916 50 916
LCA.no AS e-mail: post@lca.no
Dokka 6A, 1671 Kråkerøy, Norway web: www.lca.no
Developer of EPD generator Phone: +47 916 50 916
LCA.no AS e-mail: post@lca.no
Dokka 6A, 1671 Kråkerøy, Norway web: www.lca.no
ECO Platform web: www.eco-platform.org
ECO Portal web: ECO Portal
14 / 14
