Environmental product declaration
in accordance with ISO 14025 and EN 15804+A2
Protecta FR Pipe Wrap (pcs in plastic bag) for Sweden
Owner of the declaration: Program operator:
Polyseam AS The Norwegian EPD Foundation
Product: Declaration number:
Protecta FR Pipe Wrap (pcs in plastic bag) for Sweden
NEPD-8730-8394
Declared unit:
1 kg Registration number:
This declaration is based on Product Category Rules: NEPD-8730-8394
CEN Standard EN 15804:2012+A2:2019 serves as core
Issue date: 15.01.2025
PCR
The Norwegian EPD Foundation NPCR 009:2021 Part B for Technical - Chemical products Valid to: 15.01.2030
for building and construction industry
EPD software:
LCAno EPD generator ID: 747501
1 / 11
General information
Product Owner of the declaration:
Protecta FR Pipe Wrap (pcs in plastic bag) for Sweden Polyseam AS
Contact person: Andrea Bogstad
Phone: +47 33 30 67 00
e-mail: post.no@polyseam.com
Program operator: Manufacturer:
The Norwegian EPD Foundation Polyseam Ltd
Post Box 5250 Majorstuen, 0303 Oslo, Norway
Phone: +47 977 22 020
web: www.epd-norge.no
Declaration number: Place of production:
Polyseam Ltd
NEPD-8730-8394
St Andrews Road 15
HD1 6SB Huddersfield, West Yorkshire, United Kingdom
This declaration is based on Product Category Rules: Management system:
CEN Standard EN 15804:2012+A2:2019 serves as core PCR ISO 9001, ISO 14001
NPCR 009:2021 Part B for Technical - Chemical products for building
and construction industry
Statement of liability: Organisation no:
The owner of the declaration shall be liable for the underlying 986 426 051
information and evidence. EPD Norway shall not be liable with respect
to manufacturer information, life cycle assessment data and
evidences.​
Declared unit: Issue date:
1 kg Protecta FR Pipe Wrap (pcs in plastic bag) for Sweden 15.01.2025
Declared unit with option: Valid to:
A1,A2,A3,A4,A5,C1,C2,C3,C4,D 15.01.2030
Year of study:
2022
Functional unit: Comparability:
EPD of construction products may not be comparable if they not
comply with EN 15804 and seen in a building context.
General information on verification of EPD from EPD tools: Development and verification of EPD:
Independent verification of data, other environmental information The declaration is created using EPD tool lca.tools ver EPD2022.03,
and the declaration according to ISO 14025:2010, § 8.1.3 and § 8.1.4. developed by LCA.no. The EPD tool is integrated in the company's
Verification of each EPD is made according to EPD-Norway’s management system, and has been approved by EPD Norway.
guidelines for verification and approval requiring that tools are i)
integrated into the company's environmental management system, ii) Developer of EPD: Andrea Bogstad
the procedures for use of the EPD tool are approved by EPD-Norway,
Reviewer of company-specific input data and EPD: Jørn Davidsen
and iii) the process is reviewed annually by an independent third
party verifier. See Appendix G of EPD-Norway's General Programme
Instructions for further information on EPD tools
Verification of EPD tool: Approved:
Independent third party verification of the EPD tool, background data
and test-EPD in accordance with EPDNorway's procedures and
guidelines for verification and approval of EPD tools. NEPDT73
Third party verifier:
Elisabet Amat, GREENIZE projects
(no signature required)
2 / 11
Product
Product description:
Protecta FR Pipe Wrap is designed to maintain the fire resistance of fire separating walls and floors when these are breached by plastic pipes,
conduits or metal pipes with continuous combustible insulation. It may be used in drywalls, masonry or concrete walls and floors.
Each pipe wrap consists of a graphite-based reactive intumescent strip which reacts to heat and closes the opening left by the softening plastic
pipe or pipe insulation in a fire. It can be installed completely around the pipes or insulation and secured with the self adhesive tab. The annular
space around the pipe wrap is to be sealed with EX Mortar or FR Board.
Product specification
Materials Value Unit
MATERIALS
Binder 15-30 %
Chemical 65-85 %
Plastic - Polyethylene (LDPE) 5-10 %
PACKAGING
Packaging - Cardboard 0,02 kg
Packaging - Plastic 0,00 kg
Technical data:
The product has third-party verified ETAs and UKTAs issued in accordance with regulation (EU) No 305/2011 on the basis of EAD 350454-00-
1104, September 2017, tested to EN 1366-3, -4 & -12 in conjunction with EN 1363-1. The product hold the following approval marks; CE-mark
for Europe, UKCA mark for UK, UL-EU Certificate Internationally & UAE Certificate of Compliance.
For more information, please see https://protecta.co.uk/sv/product/fire-rated-pipe-wrap/
Market:
Sweden.
Reference service life, product
The reference service life of the product depends on its application area.
Reference service life, building
60 years.
LCA: Calculation rules
Declared unit:
1 kg Protecta FR Pipe Wrap (pcs in plastic bag) for Sweden
Cut-off criteria:
All major raw materials and all the essential energy is included. The production processes for raw materials and energy flows with very small
amounts (less than 1%) are not included. These cut-off criteria do not​ apply for hazardous materials and substances.
Allocation:
The allocation is made in accordance with the provisions of EN 15804. Incoming energy and water and waste production in-house is allocated
equally among all products through mass allocation. Effects of primary production of recycled materials is allocated to the main product in which
the material was used. The recycling process and transportation of the material is allocated to this analysis.
Data quality:
Specific data for the product composition are provided by the manufacturer. The data represent the production of the declared product and were
collected for EPD development in the year of study. Background data is based on EPDs according to EN 15804 and different LCA databases. The
data quality of the raw materials in A1 is presented in the table below.
Materials Source Data quality Year
Binder ecoinvent 3.6 Database 2019
Chemical ecoinvent 3.6 Database 2019
Packaging - Cardboard Modified ecoinvent 3.6 Database 2019
Packaging - Plastic ecoinvent 3.6 Database 2019
Plastic - Polyethylene (LDPE) ecoinvent 3.6 Database 2019
3 / 11
System boundaries (X=included, MND=module not declared, MNR=module not relevant)
Construction Beyond the system
Product stage Use stage End of life stage
installation stage boundaries
A1 A2 A3 A4 A5 B1 B2 B3 B4 B5 B6 B7 C1 C2 C3 C4 D
X X X X X MND MND MND MND MND MND MND X X X X X
System boundary:
The life cycle analysis is a cradle-to-gate (A1 - A3) study, with optional modules A4-A5, C1-C4, and D. It includes the extraction and production of
raw materials and packaging, transportation to the manufacturing site, the production process itself, transportation to the construction site, waste
management during product installation, demolition of the building, transportation to waste treatment facilities, waste treatment, as well as
potential recycling, reuse, repurposing, or energy recovery.
A4: Transportation from the factory in England to Sweden is included. Additionally, 300 km of transportation from our warehouse to the
construction site is added according to the PCR.
A5: Manual installation is assumed, and electricity consumption is not considered. A 0% material loss is included during installation. All packaging is
sent to average waste management.
C1: Average datasets are used for demolition.
C2: 50 km transport to the nearest waste treatment facility is assumed.
C3: The entire product is assumed to be sent for incineration.
C4: Ash from incineration is sent to landfill.
D: Incineration generates energy for district heating and electricity production.
Additional technical information:
Protecta FR Pipe Wrap can easily be removed and reused if the product is undamaged.
Polyseam's factory is certified according to the ISO 14001 Environmental Management Systems (EMS). It provides a framework for organisations
to design and implement an EMS, and continually improve their environmental performance.
Learn more: https://www.polyseam.com/sustainability/
waR slairetam tropsnarT gnirutcafunaM tropsnarT ylbmessA e​sU ecnanetniaM riapeR tnemecalpeR tnemhsibrufeR lanoitarepO ygrene esu lanoitarepO esu retaw -eD noitcurtsnoc noitilomed tropsnarT etsaW gnissecorp lasopsiD -yrevoceR-esueR laitnetop-gnilcyceR
4 / 11
LCA: Scenarios and additional technical information
The following information describe the scenarios in the different modules of the EPD.
Capacity utilisation Value
Transport from production place to user (A4) Distance (km) Fuel/Energy Consumption Unit
(incl. return) % (Liter/tonne)
Ship, Ferry, Sea (km) 50,0 % 1322 0,034 l/tkm 44,95
Truck, 16-32 tonnes, EURO 6 (km) - Europe 36,7 % 457 0,043 l/tkm 19,65
Truck, 16-32 tonnes, EURO 6 (km) - Europe 36,7 % 300 0,043 l/tkm 12,90
Truck, 16-32 tonnes, EURO 6 (km) - Europe 36,7 % 138 0,043 l/tkm 5,93
Assembly (A5) Unit Value
Waste, packaging, cardboard, to average
kg 0,020
treatment (kg)
Waste, packaging, plastic film (LDPE), to average
kg 0,0042
treatment (kg)
De-construction demolition (C1) Unit Value
Demolition of building and mixed material
collection, 0,012kWh per kg demolished material kg 1,000000000
(kg)
Capacity utilisation Value
Transport to waste processing (C2) Distance (km) Fuel/Energy Consumption Unit
(incl. return) % (Liter/tonne)
Truck, over 32 tonnes, EURO 6 (km) - Europe 53,3 % 50 0,023 l/tkm 1,15
Waste processing (C3) Unit Value
Waste treatment per kg Hazardous waste,
kg 1,000000000
incineration (kg)
Disposal (C4) Unit Value
Landfilling of ashes from incineration of
kg 0,18
Hazardous waste, from incineration (kg)
Benefits and loads beyond the system
Unit Value
boundaries (D)
Substitution of electricity (MJ) MJ 0,0012
Substitution of thermal energy, district heating
MJ 0,018
(MJ)
5 / 11
LCA: Results
The LCA results are presented below for the declared unit defined on page 2 of the EPD document.
Environmental impact
Indicator Unit A1 A2 A3 A4 A5 C1 C2 C3 C4 D
GWP-total
kg CO2 -
5,91E-01 2,99E-01 5,40E-02 3,15E-01 3,46E-02 4,00E-03 4,70E-03 2,22E+00 8,26E-02 -1,10E-04
eq
GWP-fossil
kg CO2 -
6,23E-01 2,99E-01 5,23E-02 3,15E-01 6,61E-04 4,00E-03 4,70E-03 2,22E+00 8,26E-02 -1,06E-04
eq
GWP-biogenic
kg CO2 -
-3,29E-02 9,85E-05 1,68E-03 1,06E-04 3,40E-02 7,50E-07 2,01E-06 5,56E-03 3,28E-05 -2,18E-07
eq
GWP-luluc
kg CO2 -
4,89E-04 1,63E-04 5,97E-05 1,54E-04 1,33E-07 3,15E-07 1,43E-06 5,59E-04 7,95E-06 -3,64E-06
eq
kg
ODP CFC11 - 2,94E-08 6,55E-08 4,67E-09 6,71E-08 8,80E-11 8,64E-10 1,13E-09 2,54E-07 4,00E-09 -7,71E-06
eq
mol H+
AP 2,52E-03 6,31E-03 1,83E-04 5,59E-03 1,95E-06 4,19E-05 1,51E-05 3,26E-03 1,63E-04 -8,72E-07
-eq
EP-FreshWater kg P -eq 1,74E-05 1,68E-06 1,34E-06 1,86E-06 3,35E-09 1,46E-08 3,74E-08 5,32E-05 8,00E-07 -9,40E-09
EP-Marine kg N -eq 4,58E-04 1,59E-03 3,70E-05 1,37E-03 8,87E-07 1,85E-05 3,31E-06 6,73E-04 4,24E-05 -2,85E-07
mol N -
EP-Terrestial 5,11E-03 1,76E-02 4,03E-04 1,52E-02 6,98E-06 2,00E-04 3,70E-05 7,59E-03 4,97E-04 -3,08E-06
eq
kg
POCP NMVOC 2,18E-03 4,65E-03 1,05E-04 4,07E-03 2,07E-06 5,57E-05 1,45E-05 2,13E-03 1,39E-04 -8,50E-07
-eq
ADP- kg Sb-
6,87E-06 4,30E-06 6,49E-07 5,41E-06 9,67E-09 6,14E-09 8,38E-08 7,74E-06 1,40E-07 -1,05E-09
minerals&metals1 eq
ADP-fossil1 MJ 1,95E+01 4,12E+00 1,07E+00 4,39E+00 5,92E-03 5,51E-02 7,63E-02 9,30E+00 3,85E-01 -1,51E-03
WDP1 m3 3,14E+01 2,13E+00 4,62E+00 2,70E+00 1,07E-02 1,17E-02 5,85E-02 3,44E+01 9,87E+00 -1,88E-02
GWP-total = Global Warming Potential total; GWP-fossil = Global Warming Potential fossil fuels; GWP-biogenic = Global Warming Potential biogenic; GWP-luluc =
Global Warming Potential land use and land use change; ODP = Depletion potential of the stratospheric ozone layer; AP = Acidification potential, Accumulated
Exceedance; EP-freshwater = Eutrophication potential, fraction of nutrients reaching freshwater end compartment: EP-marine = Eutrophication potential, fraction of
nutrients reaching marine end compartment; EP-terrestrial = Eutrophication potential, Accumulated Exceedance; POCP = Formation potential of tropospheric ozone;
ADP-minerals&metals = Abiotic depletion potential for non-fossil resources; ADP-fossil = Abiotic depletion for fossil resources potential; WDP = Water (user)
deprivation potential, deprivation-weighted water consumption
"Reading example: 9,0 E-03 = 9,0*10-3 = 0,009"
*INA Indicator Not Assessed
1. The results of this environmental impact indicator shall be used with care as the uncertainties on these results are high or as there is limited experienced with the
indicator
Remarks to environmental impacts
6 / 11
Additional environmental impact indicators
Indicator Unit A1 A2 A3 A4 A5 C1 C2 C3 C4 D
PM Disease incidence 2,27E-08 9,61E-09 7,27E-10 1,39E-08 3,00E-11 5,07E-09 4,32E-10 5,00E-08 1,10E-09 -5,20E-11
IRP2 kgBq U235 -eq 2,27E-02 1,78E-02 1,72E-02 1,90E-02 2,57E-05 2,40E-04 3,34E-04 4,23E-02 2,14E-03 -9,67E-06
ETP-fw1 CTUe 8,92E+00 2,68E+00 7,72E-01 2,91E+00 7,36E-03 3,01E-02 5,58E-02 4,51E+01 1,12E+00 -8,23E-03
HTP-c1 CTUh 1,81E-10 0,00E+00 1,90E-11 0,00E+00 0,00E+00 1,00E-12 0,00E+00 2,13E-09 6,00E-11 0,00E+00
HTP-nc1 CTUh 5,15E-09 1,54E-09 6,56E-10 3,36E-09 9,00E-12 2,80E-11 5,40E-11 1,30E-08 2,20E-09 -8,00E-12
SQP1 dimensionless 5,11E+00 1,80E+00 8,97E-01 1,92E+00 5,47E-03 6,69E-03 8,75E-02 3,67E+00 1,09E+00 -1,01E-02
PM = Particulate Matter emissions; IRP = Ionizing radiation – human health; ETP-fw = Eco toxicity – freshwater; HTP-c = Human toxicity – cancer effects; HTP-nc =
Human toxicity – non cancer effects; SQP = Potential Soil Quality Index (dimensionless)
"Reading example: 9,0 E-03 = 9,0*10-3 = 0,009"
*INA Indicator Not Assessed
1. The results of this environmental impact indicator shall be used with care as the uncertainties on these results are high or as there is limited experienced with the
indicator
2. This impact category deals mainly with the eventual impact of low dose ionizing radiation on human health of the nuclear fuel cycle. It does not consider effects due
to possible nuclear accidents, occupational exposure nor due to radioactive waste disposal in underground facilities. Potential ionizing radiation from the soil, from
radon and from some construction materials is also not measured by this indicator.
7 / 11
Resource use
Indicator Unit A1 A2 A3 A4 A5 C1 C2 C3 C4 D
PERE MJ 9,77E-01 4,07E-02 2,94E-01 4,68E-02 1,10E-04 3,00E-04 9,60E-04 1,68E+00 4,73E-02 -9,35E-03
PERM MJ 3,18E-01 0,00E+00 0,00E+00 0,00E+00 -3,18E-01 0,00E+00 0,00E+00 0,00E+00 0,00E+00 0,00E+00
PERT MJ 1,30E+00 4,07E-02 2,94E-01 4,68E-02 -3,18E-01 3,00E-04 9,60E-04 1,68E+00 4,73E-02 -9,35E-03
PENRE MJ 8,52E+00 4,12E+00 1,07E+00 4,39E+00 5,92E-03 5,51E-02 7,64E-02 9,30E+00 3,85E-01 -1,51E-03
PENRM MJ 1,17E+01 0,00E+00 0,00E+00 0,00E+00 -1,81E-01 0,00E+00 0,00E+00 0,00E+00 0,00E+00 0,00E+00
PENRT MJ 2,02E+01 4,12E+00 1,07E+00 4,39E+00 -1,75E-01 5,51E-02 7,64E-02 9,30E+00 3,85E-01 -1,51E-03
SM kg 2,69E-04 0,00E+00 0,00E+00 0,00E+00 0,00E+00 0,00E+00 0,00E+00 0,00E+00 0,00E+00 0,00E+00
RSF MJ 3,02E-02 1,28E-03 4,26E-04 1,54E-03 3,39E-06 0,00E+00 3,36E-05 3,70E-02 8,58E-04 -1,64E-06
NRSF MJ 4,42E-03 8,03E-03 4,96E-04 4,37E-03 1,26E-05 0,00E+00 1,13E-04 0,00E+00 8,48E-03 -5,54E-04
FW m3 1,16E-02 3,17E-04 4,30E-04 3,51E-04 2,87E-06 2,83E-06 8,69E-06 8,61E-03 6,85E-04 -1,13E-05
PERE = Use of renewable primary energy excluding renewable primary energy resources used as raw materials; PERM = Use of renewable primary energy resources used
as raw materials; PERT = Total use of renewable primary energy resources; PENRE = Use of non renewable primary energy excluding non-renewable primary energy
resources used as raw materials; PENRM = Use of non renewable primary energy resources used as raw materials; PENRT = Total use of non renewable primary energy
resources; SM = Use of secondary materials; RSF = Use of renewable secondary fuels; NRSF = Use of non-renewable secondary fuels; FW = Net use of fresh water
"Reading example: 9,0 E-03 = 9,0*10-3 = 0,009"
*INA Indicator Not Assessed
8 / 11
End of life - Waste
Indicator Unit A1 A2 A3 A4 A5 C1 C2 C3 C4 D
HWD kg 9,56E-04 1,93E-04 3,21E-03 2,04E-04 0,00E+00 1,62E-06 4,18E-06 0,00E+00 0,00E+00 -7,11E-08
NHWD kg 3,22E-02 1,13E-01 6,31E-03 1,20E-01 2,43E-02 6,52E-05 6,64E-03 1,00E+00 1,89E-01 -3,57E-05
RWD kg 2,09E-05 2,84E-05 8,58E-06 3,02E-05 0,00E+00 3,82E-07 5,21E-07 0,00E+00 0,00E+00 -7,92E-09
HWD = Hazardous waste disposed; NHWD = Non-hazardous waste disposed; RWD = Radioactive waste disposed
"Reading example: 9,0 E-03 = 9,0*10-3 = 0,009"
*INA Indicator Not Assessed
End of life - Output flow
Indicator Unit A1 A2 A3 A4 A5 C1 C2 C3 C4 D
CRU kg 0,00E+00 0,00E+00 0,00E+00 0,00E+00 0,00E+00 0,00E+00 0,00E+00 0,00E+00 0,00E+00 0,00E+00
MFR kg 0,00E+00 0,00E+00 1,08E-02 0,00E+00 2,08E-02 0,00E+00 0,00E+00 0,00E+00 0,00E+00 0,00E+00
MER kg 0,00E+00 0,00E+00 1,42E-02 0,00E+00 2,40E-07 0,00E+00 0,00E+00 1,00E+00 0,00E+00 0,00E+00
EEE MJ 0,00E+00 0,00E+00 8,41E-03 0,00E+00 1,14E-03 0,00E+00 0,00E+00 9,90E-04 0,00E+00 0,00E+00
EET MJ 0,00E+00 0,00E+00 1,27E-01 0,00E+00 1,73E-02 0,00E+00 0,00E+00 1,50E-02 0,00E+00 0,00E+00
CRU = Components for re-use; MFR = Materials for recycling; MER = Materials for energy recovery; EEE = Exported energy electrical; EET = Exported energy thermal
"Reading example: 9,0 E-03 = 9,0*10-3 = 0,009"
*INA Indicator Not Assessed
Biogenic Carbon Content
Indicator Unit At the factory gate
Biogenic carbon content in product kg C 0,00E+00
Biogenic carbon content in accompanying packaging kg C 9,26E-03
Note: 1 kg biogenic carbon is equivalent to 44/12 kg CO2
9 / 11
Additional requirements
Greenhouse gas emissions from the use of electricity in the manufacturing phase
National production mix from import, low voltage (production of transmission lines, in addition to direct emissions and losses in grid) of applied
electricity for the manufacturing process (A3).
Electricity mix Source Amount Unit
Electricity, United Kingdom, Market mix (kWh) ecoinvent 3.6 386,67 g CO2-eq/kWh
Electricity, United Kingdom, Solar (kWh) ecoinvent 3.6 78,98 g CO2-eq/kWh
Dangerous substances
The product contains no substances given by the REACH Candidate list.
Indoor environment
The product is fully cured upon purchase.
Properties for item FR Pipe Wrap have been declared in the Nordic Ecolabelling Building Products Portal (generation 3) and Supply Chain
Declaration Portal (generation 4).
Additional Environmental Information
Additional environmental impact indicators required in NPCR Part A for construction products
Indicator Unit A1 A2 A3 A4 A5 C1 C2 C3 C4 D
GWPIOBC kg CO2 -eq 6,03E-01 2,99E-01 6,29E-02 3,15E-01 6,61E-04 4,00E-03 4,70E-03 2,22E+00 8,26E-02 -1,08E-04
GWP-IOBC: Global warming potential calculated according to the principle of instantaneous oxidation. In order to increase the transparency of biogenic carbon​
contribution to climate impact, the indicator GWP-IOBC is required as it declares climate impacts calculated according to the principle of instantaneous oxidation.​
GWP-IOBC is also referred to as GWP-GHG in context to Swedish public procurement legislation.
10 / 11
Bibliography
ISO 14025:2010 Environmental labels and declarations - Type III environmental declarations - Principles and procedures.
ISO 14044:2006 Environmental management - Life cycle assessment - Requirements and guidelines.
EN 15804:2012+A2:2019 Environmental product declaration - Core rules for the product category of construction products.
ISO 21930:2017 Sustainability in buildings and civil engineering works - Core rules for environmental product declarations of construction
products.
ecoinvent v3, (2019) Allocation, cut-off by classification, Swiss Centre of Life Cycle Inventories.
Iversen et al., (2021) eEPD v2021.09 Background information for EPD generator tool system verification, LCA.no Report number: 07.21
Graafland, J. and Ruttenborg, M. (2023) EPD generator for NPCR009:2021, Part B for Technical - Chemical products (non-cement based products),
Background information for EPD generator application and LCA data, LCA.no report number: 12.23.
NPCR Part A: Construction products and services. Ver. 2.0, 24.03.2021 EPD Norway.
NPCR 009 Part B for Technical - Chemical products for building and construction industry, Ver. 3.0, 06.10.2021, EPD Norway.
Program operator and publisher Phone: +47 977 22 020
The Norwegian EPD Foundation e-mail: post@epd-norge.no
Post Box 5250 Majorstuen, 0303 Oslo, Norway web: www.epd-norge.no
Owner of the declaration: Phone: +47 33 30 67 00
Polyseam AS e-mail: post.no@polyseam.com
Ravneveien 7, 3174 Revetal, Norway web: https://www.polyseam.com/
Author of the Life Cycle Assessment Phone: +47 916 50 916
LCA.no AS e-mail: post@lca.no
Dokka 6A, 1671 Kråkerøy, Norway web: www.lca.no
Developer of EPD generator Phone: +47 916 50 916
LCA.no AS e-mail: post@lca.no
Dokka 6A, 1671 Kråkerøy, Norway web: www.lca.no
ECO Platform web: www.eco-platform.org
ECO Portal web: ECO Portal
11 / 11
