ver1 2015
ENVIRONMENTAL PRODUCT DECLARATION
in accordance with ISO 14025, ISO 21930 and EN 15804
Owner of the declaration: Jotun A/S
Program operator: The Norwegian EPD Foundation
Publisher: The Norwegian EPD Foundation
Declaration number: NEPD-2353-1098-EN
Registration number: NEPD-2353-1098-EN
ECO Platform reference number: -
Issue date: 07.09.2020
Valid to: 07.09.2025
Jotun Super Durable 2901, Jotun Paints (Malaysia) Sdn. Bhd.
Jotun A/S
www.epd-norge.no
NEPD-2353-1098-EN Jotun Super Durable 2901, Jotun Paints (Malaysia) Sdn. Bhd 1 / 8
General information
Product: Owner of the declaration:
Jotun Super Durable 2901, Jotun Paints (Malaysia) Sdn. Bhd.
Jotun A/S
Contact person: Anne Lill Gade
Phone: +47 33 45 70 00
e-mail: anne.lill.gade@jotun.no
Program operator: Manufacturer:
The Norwegian EPD Foundation Jotun A/S
Pb. 5250 Majorstuen, 0303 Oslo
Phone: +47 23 08 80 00
e-mail: post@epd-norge.no
Declaration number: Place of production:
Jotun Paints (Malaysia) Sdn. Bhd.
NEPD-2353-1098-EN LOT 9143, PN 38500, Kawasan Perindustrian Nilai, 71800 Nilai, Negeri Sembilan,
Malaysia.
ECO Platform reference number: Management system:
ISO 9001:2008 Certificate nr: 0044915-00, ISO 14001:2004 Certificate nr 0044914-
00, ISO 45001: 2018 Certificate nr: 0098139
This declaration is based on Product Category Rules: Organisation no:
923 248 579
CEN Standard EN 15804:2012+A1:2013 serves as core PCR.
IBU PCR Part B for coatings with organic binders
Statement of liability: Issue date:
The owner of the declaration shall be liable for the underlying information and 07.09.2020
evidence. EPD Norway shall not be liable with respect to manufacturer
information, life cycle assessment data and evidences. Valid to:
07.09.2025
Declared unit: Year of study:
1 kg Jotun Super Durable 2901, Jotun Paints (Malaysia) Sdn. Bhd. 2019
Declared unit with option: Comparability:
EPD of construction products may not be comparable if they not comply with EN
A1,A2,A3
15804 and seen in a building context.
Functional unit: Author of the Life Cycle Assessment:
The declaration is developed using eEPD v4.0 from LCA.no
Approval:
Company specific data are:
Collected/registered by: Cleo Alves Otterbech
Internal verification by: Anne Lill Gade
Verification: Approved:
Independent verification of data, other environmental information and the
declaration according to ISO14025:2010, § 8.1.3 and § 8.1.4
External
Third party verifier:
Sign
Sign
Senior Research Scientist, Anne Rønning
(Independent verifier approved by EPD Norway)
NEPD-2353-1098-EN Jotun Super Durable 2901, Jotun Paints (Malaysia) Sdn. Bhd 2 / 8
Product
Product description: Technical data:
Jotun Super Durable 2901 is a lead-free TGIC-free powder coating and it's Relative Density: 1.2 - 1.9 g/cm³.
specifically designed to meet stringent requirements of the construction Film thickness: 60-90 µm
industry. It provides longevity to the projects and building components by Recommended curing time: 10 minutes
ensuring high levels of gloss retention, colour stability and corrosion Recommended curing temperature: 200°C
protection along with aesthetic performance. The product also enables
efficient application and provides uniform flow and attractive finish even The most representative and worst case formulation produced at the
after recycling. manufacturing site is chosen for this EPD. For products with a selection of
colours, this will be the formulation with the highest content of titanium
The declared product contributes to the Green Buildings Standard credits. dioxide.
Please see section Green Building Standards. The product is highly
recommended to meet gloss retention and colour stability requirements. The product packaging is based on an average sized of a carbon box with
Primary areas of application are architectural aluminium extrusions and plastic liner.
claddings.
For safety, health and environmental conditions, see the Safety Data Sheet
When screen printing or sealants are used, it is advised to run separate trials for the declared product on www.jotun.com.
to ensure compatibility and to meet the required performance criteria.
For information on technical data, application and use of the product, see
Product specification
the Technical Data Sheet for the declared product on www.jotun.com.
For information on Green Building Standard credits, see "Additional
Information" on page 4. Market:
Global. Transport to market is not included in this EPD.
The material composition of the declared mixed product is given below:
Reference service life, product
Materials %
The reference service life of the product is highly dependent on the
Binder 50 - 75%
conditions of use. Jotun Super Durable 2901 is backed by a 25-year
Filler 10 - 25%
product guarantee system when used on an architectural aluminium
Titanium dioxide 10 - 25% substrate, subject to terms and conditions.
Additive 1 - 3%
Estimated service life, object
Pigment 1 - 3%
The coated object is not declared.
LCA: Calculation rules
Declared unit: Allocation:
The allocation is made in accordance with the provisions of EN 15804.
1 kg Jotun Super Durable 2901, Jotun Paints (Malaysia) Sdn. Bhd.
Incoming energy, water and waste production in-house is primarily
Cut-off criteria: allocated equally among all products through mass allocation. Specific
allocation was performed for certain waste flows according to information
All major raw materials and essential energy is included. The production
provided by the site manager. VOC emissions have been allocated entirely
process for raw materials and energy flows with very small amounts (less
to the production of solvent based paints. Effects of primary production of
than 0.1 % dry matter) are not included. In total, more than 99% of the
recycled materials is allocated to the main product in which the material
material input is included. These cut-off criteria do not apply for non-
was used. The recycling process and transportation of the material is
energy related emissions (such as wastes, hazardous materials and
allocated to this analysis.
substances).
Data quality:
The CEPE database is used as basis for the raw material composition. Specific data for the product composition and raw material amounts has been provided by
the manufacturer and represents the production of the declared product. Production site data was collected in 2015. Representative data from ecoinvent v3.2 was
used for other processes. The data quality for the material input in A1 is presented in tabular form.
Materials Source Data quality Year
Additives CEPE RM Database v3.0 Database 2016
Binders and Resins CEPE RM Database v3.0 Database 2016
Pigments and Fillers CEPE RM Database v3.0 Database 2016
Packaging Østfoldforskning Database 2017
NEPD-2353-1098-EN Jotun Super Durable 2901, Jotun Paints (Malaysia) Sdn. Bhd 3 / 8
System boundary:
The flowchart in the figure below illustrates the system boundaries for the analysis, in accordance with the modular principle of EN 15804. The analysis is a cradle-
to-gate (A1 - A3) study.
Additional information:
The declared product contributes to Green Building Standard credits by meeting the following specific requirements:
LEED®v4 (2013)
MR credit: Building product disclosure and optimization.
-Material Ingredients, Option 2: Material Ingredient Optimization, International Alternative Compliance Path - REACH optimization: Fully inventoried chemical
ingredients to 100 ppm and not containing substances on the REACH Authorization list – Annex XIV, the Restriction list – Annex XVII and the SVHC candidate list.
-Environmental Product Declarations. Product-specific Type III EPD (ISO 14025;21930, EN 15804) for Jotun Czech A.S. (Project Jotun Gimle) (NEPD-1564-599);
Thailand Ltd. (NEPD-1567-599); U.A.E. Ltd (LCC) (NEPD-1563-599); Jotun Boya San. ve Tic A.S. (NEPD-1566-599); PT. Jotun Indonesia (NEPD-1810-770) and Jotun
Paints (Malaysia) Sdn.Bhd.
SS Credit: Heat Island Reduction (ASTM E1980)
-Option 1: Nonroof and Roof
1.1: Non-roof (SR>0,33)
1.2.a: High-reflectance roof (Low-sloped roof, Initial SRI>82)
1.2.b: High-reflectance roof (Steep-sloped roof, Initial SRI>39)
-Option 2: Parking under Cover (Initial SRI>39)
*The following colors of the Cool Shades Collection complies:
Arc: 1.1;1.2.b;2
Couronne: 1.1;1.2.b;2
Dayspring: 1.1;1.2.b;2
Equinox: 1.1;1.2.b;2
Meridian: 1.1;1.2.a;1.2.b;2
Sepia: 1.1;1.2.b;2
Starfall: 1.1
Sun path: 1.1;1.2.a;1.2.b;2
BREEAM International (2016)
-Mat 01: Product-specific Type III EPD (ISO 14025;21930, EN 15804) for Jotun Czech A.S. (Project Jotun Gimle) (NEPD-1564-599); Thailand Ltd. (NEPD-1567-599);
U.A.E. Ltd (LCC) (NEPD-1563-599); Jotun Boya San. ve Tic A.S. (NEPD-1566-599); PT. Jotun Indonesia (NEPD-1810-770) and Jotun Paints (Malaysia) Sdn.Bhd.
Additional certificates and approvals may be available on request.
NEPD-2353-1098-EN Jotun Super Durable 2901, Jotun Paints (Malaysia) Sdn. Bhd 4 / 8
LCA: Scenarios and additional technical information
The following information describe the scenarios in the different modules of the EPD.
This is a cradle to gate (A1-A3) EPD with no declared modules after the factory gate. Transport from place of production to user (A4) has to be calculated by the
user.
NEPD-2353-1098-EN Jotun Super Durable 2901, Jotun Paints (Malaysia) Sdn. Bhd 5 / 8
LCA: Results
System boundaries (X=included, MND=module not declared, MNR=module not relevant)
Construction Beyond the
Product stage installation User stage End of life stage . system
stage bondaries
A1 A2 A3 A4 A5 B1 B2 B3 B4 B5 B6 B7 C1 C2 C3 C4 . D
X X X MND MND MND MND MND MND MND MND MND MND MND MND MND . MND
Environmental impact
Parameter Unit A1 A2 A3
GWP kg CO 2 -eq 4,94E+00 1,26E-01 9,54E-01
ODP kg CFC11 -eq 4,24E-06 2,25E-08 3,01E-08
POCP kg C 2H 4-eq 2,33E-03 7,55E-05 1,87E-04
AP kg SO 2 -eq 2,22E-02 2,31E-03 4,53E-03
EP kg PO 3- -eq 5,01E-03 2,53E-04 1,42E-03
4
ADPM kg Sb -eq 1,31E-05 5,73E-08 5,85E-07
ADPE MJ 8,86E+01 1,87E+00 1,19E+01
GWP Global warming potential; ODP Depletion potential of the stratospheric ozone layer; POCP Formation potential of tropospheric photochemical oxidants;
AP Acidification potential of land and water; EP Eutrophication potential; ADPM Abiotic depletion potential for non fossil resources; ADPE Abiotic depletion
potential for fossil resources
Reading example: 9,0 E-03 = 9,0*10-3 = 0,009
*INA Indicator Not Assessed
waR slairetam tropsnarT gnirutcafunaM tropsnarT ylbmessA esU ecnanetniaM riapeR tnemecalpeR tnemhsibrufeR lanoitarepO ygrene esu lanoitarepO esu
retaw
-eD noitcurtsnoc noitilomed tropsnarT etsaW gnissecorp lasopsiD -yrevoceR-esueR -gnilcyceR laitnetop
NEPD-2353-1098-EN Jotun Super Durable 2901, Jotun Paints (Malaysia) Sdn. Bhd 6 / 8
Resource use
Parameter Unit A1 A2 A3
RPEE MJ 3,63E+00 4,11E-02 7,80E-01
RPEM MJ 1,39E+00 8,16E-03 1,21E-01
TPE MJ 5,03E+00 4,92E-02 9,01E-01
NRPE MJ 9,88E+01 1,94E+00 1,20E+01
NRPM MJ 0,00E+00 0,00E+00 0,00E+00
TRPE MJ 9,88E+01 1,94E+00 1,20E+01
SM kg 0,00E+00 0,00E+00 0,00E+00
RSF MJ 0,00E+00 0,00E+00 0,00E+00
NRSF MJ 0,00E+00 0,00E+00 0,00E+00
W m3 3,68E-01 2,87E-04 3,23E-03
RPEE Renewable primary energy resources used as energy carrier; RPEM Renewable primary energy resources used as raw materials; TPE Total use of renewable
primary energy resources; NRPE Non renewable primary energy resources used as energy carrier; NRPM Non renewable primary energy resources used as
materials; TRPE Total use of non renewable primary energy resources; SM Use of secondary materials; RSF Use of renewable secondary fuels; NRSF Use of non
renewable secondary fuels; W Use of net fresh water
Reading example: 9,0 E-03 = 9,0*10-3 = 0,009
*INA Indicator Not Assessed
End of life - Waste
Parameter Unit A1 A2 A3
HW kg 1,31E-03 1,04E-06 4,45E-06
NHW kg 1,31E+00 4,52E-02 6,70E-01
RW kg INA* INA* INA*
HW Hazardous waste disposed; NHW Non hazardous waste disposed; RW Radioactive waste disposed
Reading example: 9,0 E-03 = 9,0*10-3 = 0,009
*INA Indicator Not Assessed
End of life - Output flow
Parameter Unit A1 A2 A3
CR kg 0,00E+00 0,00E+00 0,00E+00
MR kg 0,00E+00 0,00E+00 2,96E-02
MER kg 0,00E+00 0,00E+00 1,30E-02
EEE MJ INA* INA* INA*
ETE MJ INA* INA* INA*
CR Components for reuse; MR Materials for recycling; MER Materials for energy recovery; EEE Exported electric energy; ETE Exported thermal energy
Reading example: 9,0 E-03 = 9,0*10-3 = 0,009
*INA Indicator Not Assessed
NEPD-2353-1098-EN Jotun Super Durable 2901, Jotun Paints (Malaysia) Sdn. Bhd 7 / 8
Additional requirements
Greenhouse gas emissions from the use of electricity in the manufacturing phase
National production mix from import, low voltage (production of transmission lines, in addition to direct emissions and losses in grid) of applied electricity for the
manufacturing process (A3).
Electricity mix Data source Amount Unit
Electricity, Malaysia (kWh) ecoinvent 3.3 Alloc Rec 861,04 g CO2-ekv/kWh
Dangerous substances
The product contains no substances given by the REACH Candidate list.
Indoor environment
Jotun powder coatings do not emit volatile organic substances (VOC) after application.
Bibliography
ISO 14025:2010 Environmental labels and declarations - Type III environmental declarations - Principles and procedures.
ISO 14044:2006 Environmental management - Life cycle assessment - Requirements and guidelines.
EN 15804:2012+A1:2013 Environmental product declaration - Core rules for the product category of construction products.
ISO 21930:2017 Sustainability in buildings and civil engineering works - Core rules for environmental product declarations of construction products.
IBU PCR Part B: Requirements on the EPD for Coatings with organic binders. v1.4, September 2016.
Vold et al (2017). EPD and LCA tool for Jotun - Technical description and background information, OR 01.17, Ostfold Research, Fredrikstad 2017.
CEPE v3.0 Raw materials LCI database for the European coatings and printing ink industries, May 2016.
ecoinvent v3.2 Alloc Rec, Swiss Centre of Life Cycle Inventories.
ASTM E1980-11 (2001): Standard Practice for Calculating Solar Reflectance Index of Horizontal and Low-Sloped Opaque Surfaces, ASTM International, West Conshohocken, PA.
BREEAM International (2016): BREEAM International New Construction Technical Manual. SD233-2.0:2017.
LEED®v4 (2013): LEED® v4 for Building design and construction, U.S. Green Building Council®.
REACH (2006): Regulation (EC) No 1907/2006 of the European Parliament and of the Council of 18 December 2006. REACH Authorization list – Annex XIV, the Restriction list –
Annex XVII and the SVHC candidate list.
Program operator and publisher Phone: +47 23 08 80 00
The Norwegian EPD Foundation
Post Box 5250 Majorstuen, 0303 Oslo e-mail: post@epd-norge.no
0303 Oslo Norway web: www.epd-norge.no
Owner of the declaration Phone: +47 33 45 70 00
Jotun A/S Fax:
Hystadveien 167 e-mail: anne.lill.gade@jotun.no
3209 Sandefjord web: www.jotun.no
Author of the Life Cycle Assessment Phone: +47 69 35 11 00
Østfoldforskning AS Fax: +47 69 34 24 94
Stadion 4 e-mail:
1671 Kråkerøy web: www.ostfoldforskning.no
Developer of EPD generator Phone: +47 916 50 916
LCA.no AS
Dokka 1C e-mail: post@lca.no
1671 Kråkerøy web: www.lca.no
NEPD-2353-1098-EN Jotun Super Durable 2901, Jotun Paints (Malaysia) Sdn. Bhd 8 / 8
