Environmental product declaration
in accordance with ISO 14025 and EN 15804+A2
Protecta FR Board 1-S for Sweden
Owner of the declaration: Program operator:
Polyseam AS The Norwegian EPD Foundation
Product: Declaration number:
Protecta FR Board 1-S for Sweden
Registration number:
Declared unit:
1 m2 Issue date:
This declaration is based on Product Category Rules: Valid to:
CEN Standard EN 15804:2012+A2:2019 serves as core
EPD software:
PCR.
The Norwegian EPD Foundation LCAno EPD generator ID: 415265
NPCR 012:2022 Part B for Thermal insulation products
1 / 11
General information
Product Owner of the declaration:
Protecta FR Board 1-S for Sweden Polyseam AS
Contact person: Andrea Bogstad
Phone: +47 33 30 67 00
e-mail: post.no@polyseam.com
Program operator: Manufacturer:
The Norwegian EPD Foundation Polyseam Ltd
Post Box 5250 Majorstuen, 0303 Oslo, Norway
Phone: +47 977 22 020
web: www.epd-norge.no
Declaration number: Place of production:
Polyseam Ltd
St Andrews Road 15
HD1 6SB Huddersfield, West Yorkshire, United Kingdom
This declaration is based on Product Category Rules: Management system:
CEN Standard EN 15804:2012+A2:2019 serves as core PCR. ISO 9001, ISO 14001
NPCR 012:2022 Part B for Thermal insulation products
Statement of liability: Organisation no:
The owner of the declaration shall be liable for the underlying 986 426 051
information and evidence. EPD Norway shall not be liable with respect
to manufacturer information, life cycle assessment data and
evidences.​
Declared unit: Issue date:
1 m2 Protecta FR Board 1-S for Sweden
Declared unit with option: Valid to:
A1,A2,A3,A4,A5,C1,C2,C3,C4,D
Year of study:
2022
Functional unit: Comparability:
1 m2 Protecta FR Board with top coating on one side. The board is EPD of construction products may not be comparable if they not
50mm thick and has a 160 kg/m3 density. Density of coating: 1,3-1,4 comply with EN 15804:2012+A2:2019 and seen in a building context.
kg/ltr. Thermal conductivity: 0,038 W/mK.
General information on verification of EPD from EPD tools: Development and verification of EPD:
Independent verification of data, other environmental information The declaration is created using EPD tool lca.tools ver EPD2022.03,
and the declaration according to ISO 14025:2010, § 8.1.3 and § 8.1.4. developed by LCA.no. The EPD tool is integrated in the company's
Verification of each EPD is made according to EPD-Norway’s management system, and has been approved by EPD Norway.
guidelines for verification and approval requiring that tools are i)
integrated into the company's environmental management system, ii) Developer of EPD: Andrea Bogstad
the procedures for use of the EPD tool are approved by EPD-Norway,
Reviewer of company-specific input data and EPD:​ Jørn Davidsen
and iii) the process is reviewed annually by an independent third
party verifier. See Appendix G of EPD-Norway's General Programme
Instructions for further information on EPD tools
Verification of EPD tool: Approved:
Independent third party verification of the EPD tool, background data
and test-EPD in accordance with EPDNorway's procedures and
guidelines for verification and approval of EPD tools.
Third party verifier:
Elisabet Amat, GREENIZE projects
(no signature required)
2 / 11
Product
Product description:
Protecta FR Board is designed to prevent the spread of fire and smoke through openings in fire rated walls and floors where openings are formed
to allow the installation of multiple building services. FR Board will also maintain the acoustic designed performance in fire rated walls and floors.
FR Board consists of a high density, stone wool core which is over-coated with FR Coating. The top coating provides additional protection by
significantly reducing the permeability of the stone wool core and prevents the passage of hot gases, thus reducing the temperature rise on the
unexposed side and reducing heat conduction through the building services.
FR Board is available with top coating on one or two sides, selected on the basis of installation considerations and fire resistance. On site, FR Board
must be used together with FR Acrylic for sealing around building services and the surrounding construction.
Product specification
Materials Value Unit
MATERIALS
Paint 15-20 %
Mineral 80-90 %
PACKAGING
Packaging - Wood 0,19 kg
Packaging - Plastic 0,09 kg
Technical data:
The product has third-party verified ETAs issued in accordance with regulation (EU) No 305/2011 on the basis of EAD 350454-00-1104, tested to
EN 1366-1, -3, -4 & -12 in conjunction with EN 1363-1. The product is CE-marked for Europe.
For more information, please see https://www.protecta.no/sv/product/fr-board/
Market:
Sweden.
Reference service life, product
60 years, if installed correctly.
Reference service life, building or construction works
60 years.
LCA: Calculation rules
Declared unit:
1 m2 Protecta FR Board 1-S for Sweden
Cut-off criteria:
All major raw materials and all the essential energy is included. The production processes for raw materials and energy flows with very small
amounts (less than 1%) are not included. These cut-off criteria do not apply for hazardous materials and substances.
Allocation:
The allocation is made in accordance with the provisions of EN 15804+A2. Incoming energy and water and waste production in-house is allocated
equally among all products through mass allocation. Effects of primary production of recycled materials is allocated to the main product in which
the material was used. The recycling process and transportation of the material is allocated to this analysis.
Data quality:
Specific data for the product composition are provided by the manufacturer. The data represent the production of the declared product and were
collected for EPD development in the year of study. Background data is based on EPDs according to EN 15804 and different LCA databases. The
data quality of the raw materials in A1 is presented in the table below.
Materials Source Data quality Year
Mineral ecoinvent 3.6 Database 2019
Packaging - Plastic ecoinvent 3.6 Database 2019
Packaging - Wood Modified ecoinvent 3.6 Database 2019
Chemical ecoinvent 3.6 Database 2019
Chemical Modified ecoinvent 3.6 Database 2019
Solvent ecoinvent 3.6 Database 2019
Binder ecoinvent 3.6 Database 2019
Pigments ecoinvent 3.6 Database 2019
Packaging - Paper ecoinvent 3.6 Database 2019
Preservative ecoinvent 3.6 Database 2019
3 / 11
System boundaries (X=included, MND=module not declared, MNR=module not relevant)
Construction Beyond the system
Product stage Use stage End of life stage
installation stage boundaries
A1 A2 A3 A4 A5 B1 B2 B3 B4 B5 B6 B7 C1 C2 C3 C4 D
X X X X X MND MND MND MND MND MND MND X X X X X
System boundary:
The life cycle analysis is a cradle-to-grave study, excluding the use phase (B1-B7). It includes the extraction and production of raw materials and
packaging, transportation to the manufacturing site, the production process itself, transportation to the construction site, waste management
during product installation, demolition, transportation to waste treatment, the waste treatment process, landfill of materials, as well as avoided
emissions and resource use in a new product.
A4: Transportation from the factory in England to Sweden is included. Additionally, 300 km of transportation from our warehouse to the
construction site is added according to the PCR.
A5: Manual installation is assumed, and electricity is not accounted for. No sealants/adhesives are included. Our fire-rated products are system-
approved and have EPDs for the necessary products. We expect the EPDs for the used products to be attached as documentation. 2% material
waste is included during installation. All packaging is sent for average waste management.
C1: Average datasets are used for demolition.
C2: 50 km of transportation to the nearest waste treatment facility is assumed.
C3: No part of the product is assumed to be sent for incineration.
C4: The entire product is assumed to be sent to landfill. The stone wool can be recycled if the paint is removed. However, we consider the likelihood
of this practice being carried out to be minimal.
D: Reuse, recovery, and recycling are set to zero.
Additional technical information:
Protecta FR Board can be easily removed by unscrewing the attached screws. If the product is undamaged, it can be reused. In case of paint
flaking, it can be repaired using Protecta FR Coating.
Polyseam's factory is certified according to the ISO 14001 Environmental Management Systems (EMS). It provides a framework for organisations
to design and implement an EMS, and continually improve their environmental performance.
Learn more: https://www.polyseam.com/sustainability/
waR slairetam tropsnarT gnirutcafunaM tropsnarT ylbmessA e​sU ecnanetniaM riapeR tnemecalpeR tnemhsibrufeR lanoitarepO ygrene esu lanoitarepO esu retaw -eD noitcurtsnoc noitilomed tropsnarT etsaW gnissecorp lasopsiD -yrevoceR-esueR laitnetop-gnilcyceR
4 / 11
LCA: Scenarios and additional technical information
The following information describe the scenarios in the different modules of the EPD.
Capacity utilisation Value
Transport from production place to user (A4) Distance (km) Fuel/Energy Consumption Unit
(incl. return) % (Liter/tonne)
Ship, Ferry, Sea (km) 50,0 % 1322 0,034 l/tkm 44,95
Truck, 16-32 tonnes, EURO 6 (km) - Europe 36,7 % 457 0,043 l/tkm 19,65
Truck, 16-32 tonnes, EURO 6 (km) - Europe 36,7 % 300 0,043 l/tkm 12,90
Truck, 16-32 tonnes, EURO 6 (km) - Europe 36,7 % 138 0,043 l/tkm 5,93
Assembly (A5) Unit Value
Material loss during instalation (kg) Units/DU 0,18
Waste treatment of material lost during
kg/DU 0,18
instalation (kg)
Waste, packaging, pallet, EUR wooden pallet,
kg 0,19
reusable, to average treatment (kg)
Waste, packaging, plastic film (LDPE), to average
kg 0,09
treatment (kg)
De-construction demolition (C1) Unit Value
Demolition of building and mixed material
collection, 0,012kWh per kg demolished material kg/DU 9,17
(kg)
Capacity utilisation Value
Transport to waste processing (C2) Distance (km) Fuel/Energy Consumption Unit
(incl. return) % (Liter/tonne)
Truck, over 32 tonnes, EURO 6 (km) - Europe 53,3 % 50 0,023 l/tkm 1,15
Disposal (C4) Unit Value
Waste, paint, to landfill (kg) kg/DU 1,39
Waste, stone wool, to landfil (kg) kg/DU 7,50
5 / 11
LCA: Results
The LCA results are presented below for the declared unit defined on page 2 of the EPD document.
Environmental impact
Indicator Unit A1 A2 A3 A4 A5 C1 C2 C3 C4 D
GWP-total
kg CO2 -
9,85E+00 1,52E-01 4,80E-01 2,67E+00 5,07E-01 3,67E-02 4,00E-02 0 2,02E-01 0
eq
GWP-fossil
kg CO2 -
1,02E+01 1,52E-01 4,65E-01 2,67E+00 2,17E-01 3,67E-02 3,99E-02 0 2,02E-01 0
eq
GWP-biogenic
kg CO2 -
-3,71E-01 6,28E-05 1,50E-02 8,99E-04 2,90E-01 6,88E-06 1,71E-05 0 4,01E-05 0
eq
GWP-luluc
kg CO2 -
7,67E-03 5,36E-05 5,30E-04 1,31E-03 1,54E-04 2,89E-06 1,22E-05 0 1,39E-05 0
eq
kg
ODP CFC11 - 6,83E-07 3,44E-08 4,15E-08 5,70E-07 2,36E-08 7,92E-09 9,63E-09 0 2,06E-08 0
eq
mol H+
AP 9,38E-02 4,39E-04 1,63E-03 4,75E-02 3,67E-04 3,84E-04 1,29E-04 0 4,76E-04 0
-eq
EP-FreshWater kg P -eq 3,71E-04 1,21E-06 1,19E-05 1,58E-05 5,15E-06 1,34E-07 3,18E-07 0 5,74E-07 0
EP-Marine kg N -eq 9,08E-03 8,78E-05 3,29E-04 1,16E-02 8,38E-05 1,69E-04 2,82E-05 0 1,67E-04 0
mol N -
EP-Terrestial 1,58E-01 9,81E-04 3,58E-03 1,29E-01 8,80E-04 1,83E-03 3,14E-04 0 1,84E-03 0
eq
kg
POCP NMVOC 4,85E-02 3,75E-04 9,31E-04 3,45E-02 2,74E-04 5,11E-04 1,23E-04 0 5,67E-04 0
-eq
ADP- kg Sb-
8,79E-05 4,12E-06 5,74E-06 4,60E-05 8,47E-07 5,63E-08 7,11E-07 0 4,65E-07 0
minerals&metals1 eq
ADP-fossil1 MJ 1,53E+02 2,30E+00 9,48E+00 3,73E+01 1,02E+00 5,05E-01 6,49E-01 0 1,42E+00 0
WDP1 m3 1,66E+03 2,20E+00 4,10E+01 2,29E+01 4,00E+00 1,07E-01 4,97E-01 0 2,38E+00 0
GWP-total = Global Warming Potential total; GWP-fossil = Global Warming Potential fossil fuels; GWP-biogenic = Global Warming Potential biogenic; GWP-luluc =
Global Warming Potential land use and land use change; ODP = Depletion potential of the stratospheric ozone layer; AP = Acidification potential, Accumulated
Exceedance; EP-freshwater = Eutrophication potential, fraction of nutrients reaching freshwater end compartment: EP-marine = Eutrophication potential, fraction of
nutrients reaching marine end compartment; EP-terrestrial = Eutrophication potential, Accumulated Exceedance; POCP = Formation potential of tropospheric ozone;
ADP-minerals&metals = Abiotic depletion potential for non-fossil resources; ADP-fossil = Abiotic depletion for fossil resources potential; WDP = Water (user)
deprivation potential, deprivation-weighted water consumption
"Reading example: 9,0 E-03 = 9,0*10-3 = 0,009"
*INA Indicator Not Assessed
1. The results of this environmental impact indicator shall be used with care as the uncertainties on these results are high or as there is limited experienced with the
indicator
Remarks to environmental impacts
6 / 11
Additional environmental impact indicators
Indicator Unit A1 A2 A3 A4 A5 C1 C2 C3 C4 D
PM Disease incidence 5,12E-07 9,48E-09 6,45E-09 1,18E-07 5,70E-09 4,64E-08 3,67E-09 0 9,44E-09 0
IRP2 kgBq U235 -eq 3,89E-01 1,00E-02 1,53E-01 1,62E-01 4,28E-03 2,20E-03 2,83E-03 0 5,98E-03 0
ETP-fw1 CTUe 2,09E+02 1,70E+00 6,86E+00 2,47E+01 4,32E+00 2,76E-01 4,74E-01 0 8,48E-01 0
HTP-c1 CTUh 3,86E-08 0,00E+00 1,72E-10 0,00E+00 2,41E-10 9,00E-12 0,00E+00 0 3,20E-11 0
HTP-nc1 CTUh 1,29E-07 1,85E-09 5,83E-09 2,85E-08 1,73E-09 2,57E-10 4,58E-10 0 6,73E-10 0
SQP1 dimensionless 1,01E+02 1,65E+00 7,95E+00 1,63E+01 8,12E-01 6,13E-02 7,43E-01 0 3,46E+00 0
PM = Particulate Matter emissions; IRP = Ionizing radiation – human health; ETP-fw = Eco toxicity – freshwater; HTP-c = Human toxicity – cancer effects; HTP-nc =
Human toxicity – non cancer effects; SQP = Potential Soil Quality Index (dimensionless)
"Reading example: 9,0 E-03 = 9,0*10-3 = 0,009"
*INA Indicator Not Assessed
1. The results of this environmental impact indicator shall be used with care as the uncertainties on these results are high or as there is limited experienced with the
indicator
2. This impact category deals mainly with the eventual impact of low dose ionizing radiation on human health of the nuclear fuel cycle. It does not consider effects due
to possible nuclear accidents, occupational exposure nor due to radioactive waste disposal in underground facilities. Potential ionizing radiation from the soil, from
radon and from some construction materials is also not measured by this indicator.
7 / 11
Resource use
Indicator Unit A1 A2 A3 A4 A5 C1 C2 C3 C4 D
PERE MJ 1,96E+01 3,27E-02 2,60E+00 3,97E-01 1,94E-01 2,75E-03 8,16E-03 0 2,06E-02 0
PERM MJ 3,59E+00 0,00E+00 0,00E+00 0,00E+00 -2,65E+00 0,00E+00 0,00E+00 0 0,00E+00 0
PERT MJ 2,32E+01 3,27E-02 2,60E+00 3,97E-01 -2,46E+00 2,75E-03 8,16E-03 0 2,06E-02 0
PENRE MJ 1,31E+02 2,30E+00 9,48E+00 3,73E+01 1,02E+00 5,05E-01 6,49E-01 0 1,42E+00 0
PENRM MJ 2,41E+01 0,00E+00 0,00E+00 0,00E+00 -3,74E+00 0,00E+00 0,00E+00 0 0,00E+00 0
PENRT MJ 1,55E+02 2,30E+00 9,48E+00 3,73E+01 -2,71E+00 5,05E-01 6,49E-01 0 1,42E+00 0
SM kg 1,72E-01 0,00E+00 0,00E+00 0,00E+00 0,00E+00 0,00E+00 0,00E+00 0 2,99E-04 0
RSF MJ 2,61E-01 1,17E-03 3,79E-03 1,31E-02 3,36E-03 0,00E+00 2,85E-04 0 4,50E-04 0
NRSF MJ 8,06E-02 4,17E-03 4,41E-03 3,71E-02 1,09E-02 0,00E+00 9,56E-04 0 1,56E-03 0
FW m3 1,14E-01 2,47E-04 3,82E-03 2,99E-03 8,48E-04 2,60E-05 7,38E-05 0 1,57E-03 0
PERE = Use of renewable primary energy excluding renewable primary energy resources used as raw materials; PERM = Use of renewable primary energy resources used
as raw materials; PERT = Total use of renewable primary energy resources; PENRE = Use of non renewable primary energy excluding non-renewable primary energy
resources used as raw materials; PENRM = Use of non renewable primary energy resources used as raw materials; PENRT = Total use of non renewable primary energy
resources; SM = Use of secondary materials; RSF = Use of renewable secondary fuels; NRSF = Use of non-renewable secondary fuels; FW = Net use of fresh water
"Reading example: 9,0 E-03 = 9,0*10-3 = 0,009"
*INA Indicator Not Assessed
8 / 11
End of life - Waste
Indicator Unit A1 A2 A3 A4 A5 C1 C2 C3 C4 D
HWD kg 1,89E-02 1,19E-04 2,85E-02 1,73E-03 1,78E-01 1,49E-05 3,55E-05 0 8,56E-05 0
NHWD kg 8,55E-01 1,16E-01 5,61E-02 1,02E+00 9,76E-02 5,98E-04 5,64E-02 0 8,89E+00 0
RWD kg 3,02E-04 1,57E-05 7,63E-05 2,57E-04 0,00E+00 3,51E-06 4,43E-06 0 7,25E-06 0
HWD = Hazardous waste disposed; NHWD = Non-hazardous waste disposed; RWD = Radioactive waste disposed
"Reading example: 9,0 E-03 = 9,0*10-3 = 0,009"
*INA Indicator Not Assessed
End of life - Output flow
Indicator Unit A1 A2 A3 A4 A5 C1 C2 C3 C4 D
CRU kg 0,00E+00 0,00E+00 0,00E+00 0,00E+00 1,81E-01 0,00E+00 0,00E+00 0 0,00E+00 0
MFR kg 5,78E-02 0,00E+00 9,80E-02 0,00E+00 8,26E-02 0,00E+00 0,00E+00 0 2,81E-04 0
MER kg 2,18E-02 0,00E+00 7,78E-07 0,00E+00 9,44E-02 0,00E+00 0,00E+00 0 2,27E-06 0
EEE MJ 4,22E-02 0,00E+00 7,48E-02 0,00E+00 6,70E-03 0,00E+00 0,00E+00 0 1,96E-05 0
EET MJ 6,39E-01 0,00E+00 1,13E+00 0,00E+00 1,01E-01 0,00E+00 0,00E+00 0 2,97E-04 0
CRU = Components for re-use; MFR = Materials for recycling; MER = Materials for energy recovery; EEE = Exported energy electrical; EET = Exported energy thermal
"Reading example: 9,0 E-03 = 9,0*10-3 = 0,009"
*INA Indicator Not Assessed
Biogenic Carbon Content
Indicator Unit At the factory gate
Biogenic carbon content in product kg C 0,00E+00
Biogenic carbon content in accompanying packaging kg C 1,06E-01
Note: 1 kg biogenic carbon is equivalent to 44/12 kg CO2
9 / 11
Additional requirements
Greenhouse gas emissions from the use of electricity in the manufacturing phase
National production mix from import, low voltage (production of transmission lines, in addition to direct emissions and losses in grid) of applied
electricity for the manufacturing process (A3).
Electricity mix Source Amount Unit
Electricity, United Kingdom, Market mix (kWh) ecoinvent 3.6 386,67 g CO2-eq/kWh
Electricity, United Kingdom, Solar (kWh) ecoinvent 3.6 78,98 g CO2-eq/kWh
Dangerous substances
The product contains no substances given by the REACH Candidate list.
Indoor environment
Protecta FR Board has been emission tested by Normec Product Testing. Meets the exemplary level criteria for indoor air quality as specified in
BREEAM-SE Nybyggnad v6.0.
Properties for item FR Board have been declared in the Nordic Ecolabelling Building Products Portal (generation 3) and Supply Chain Declaration
Portal (generation 4).
Additional Environmental Information
Additional environmental impact indicators required in NPCR Part A for construction products
Indicator Unit A1 A2 A3 A4 A5 C1 C2 C3 C4 D
GWPIOBC kg CO2 -eq 1,02E+01 1,52E-01 5,47E-01 2,67E+00 2,17E-01 3,67E-02 4,00E-02 0 3,95E-02 0
GWP-IOBC: Global warming potential calculated according to the principle of instantaneous oxidation. In order to increase the transparency of biogenic carbon​
contribution to climate impact, the indicator GWP-IOBC is required as it declares climate impacts calculated according to the principle of instantaneous oxidation.​
GWP-IOBC is also referred to as GWP-GHG in context to Swedish public procurement legislation.
10 / 11
Bibliography
ISO 14025:2010 Environmental labels and declarations - Type III environmental declarations - Principles and procedures.
ISO 14044:2006 Environmental management - Life cycle assessment - Requirements and guidelines.
EN 15804:2012+A2:2019 Environmental product declaration - Core rules for the product category of construction products.
ISO 21930:2017 Sustainability in buildings and civil engineering works - Core rules for environmental product declarations of construction
products.
ecoinvent v3, Allocation, cut-off by classification, Swiss Centre of Life Cycle Inventories.
Iversen et al., (2021) eEPD v2021.09 Background information for EPD generator tool system verification, LCA.no Report number: 07.21
Vold et. al., (2022) EPD generator for NPCR 012 Thermal insulation, Background information for EPD generator application and LCA data, LCA.no
report number: 07.22.
NPCR Part A: Construction products and services. Ver. 2.0. April 2021, EPD-Norge.
NPCR 012 Part B for Part B for Thermal insulation products, Ver. 2.0, 31.03.2022, EPD Norway.
SPT2023-R076 - VOC Emission Test Report
Program operator and publisher Phone: +47 977 22 020
The Norwegian EPD Foundation e-mail: post@epd-norge.no
Post Box 5250 Majorstuen, 0303 Oslo, Norway web: www.epd-norge.no
Owner of the declaration: Phone: +47 33 30 67 00
Polyseam AS e-mail: post.no@polyseam.com
Ravneveien 7, 3174 Revetal web: https://www.polyseam.com/
Author of the Life Cycle Assessment Phone: +47 916 50 916
LCA.no AS e-mail: post@lca.no
Dokka 6A, 1671 web: www.lca.no
Developer of EPD generator Phone: +47 916 50 916
LCA.no AS e-mail: post@lca.no
Dokka 6B,1671 Kråkerøy web: www.lca.no
ECO Platform web: www.eco-platform.org
ECO Portal web: ECO Portal
11 / 11
