ver1 2015
ENVIRONMENTAL PRODUCT DECLARATION
in accordance with ISO 14025, ISO 21930 and EN 15804
Owner of the declaration: Saferoad Sverige AB
Program operator: The Norwegian EPD Foundation
Publisher: The Norwegian EPD Foundation
Declaration number: NEPD-3793-2725-EN
Registration number: NEPD-3793-2725-EN
ECO Platform reference number: -
Issue date: 06.10.2022
Valid to: 06.10.2027
Birsta 3PH2b, W3, kantbalk A & B h1,2
Saferoad Sverige AB
www.epd-norge.no
NEPD-3793-2725-EN Birsta 3PH2b, W3, kantbalk A & B h1,2
1 / 8
General information
Product: Owner of the declaration:
Birsta 3PH2b, W3, kantbalk A & B h1,2 Saferoad Sverige AB
Contact person: Ulf Sköld
Phone: +46 70200648
e-mail: ulf.skold@saferoad.se
Program operator: Manufacturer:
Saferoad Sverige AB
The Norwegian EPD Foundation
Pb. 5250 Majorstuen, 0303 Oslo
Phone: +47 23 08 80 00
e-mail: post@epd-norge.no
Declaration number: Place of production:
Saferoad Sverige AB
NEPD-3793-2725-EN Volvogatan 2 731 36 Köping
Sweden
ECO Platform reference number: Management system:
ISO 9001:2015 and ISO 14001:2015, Sert no. 2615, AB, SE
This declaration is based on Product Category Rules: Organisation no:
556030-8073
CEN Standard EN 15804:2012+A1:2013 serves as core PCR
NPCR 013:2019 Part B for Steel and aluminium construction products
Statement of liability: Issue date: 06.10.2022
The owner of the declaration shall be liable for the underlying information and
evidence. EPD Norway shall not be liable with respect to manufacturer Valid to: 06.10.2027
information, life cycle assessment data and evidences.
Declared unit: Year of study:
1 m Birsta 3PH2b, W3, kantbalk A & B h1,2 2020
Declared unit with option: Comparability:
EPD of construction products may not be comparable if they not comply with EN
A1,A2,A3,A4,A5,C1,C2,C3,C4,D
15804 and seen in a building context.
Functional unit: Development and verification of EPD:
The declaration has been developed and verified using EPD tool lca.tools
ver EPD2020.11, developed by LCA.no AS. The EPD tool is integrated into
the company's environmental management system, and has been
approved by EPD-Norway
General information on verification of EPD from EPD tools:
Independent verification of data, other environmental information and Developer of EPD:
the declaration according to ISO 14025:2010, § 8.1.3 and § 8.1.4. Individual
third party verification of each EPD is not required when the EPD tool is i) Ulf Sköld
integrated into the company's environmental management system, ii) the
procedures for use of the EPD tool are approved by EPDNorway, and iii) Reviewer of company-specific input data and EPD:
the proccess is reviewed annualy. See Appendix G of EPD-Norway's
General Programme Instructions for further information on EPD tools. Håkan Galin
Verification of EPD tool: Approved:
Independent third party verification of the EPD tool, background data
Sign
and test-EPD in accordance with EPDNorway's procedures and guidelines
for verification and approval of EPD tools.
Martin Erlandsson, IVL Swedish Environmental Research Institute
(no signature required) Håkon Hauan, CEO EPD-Norge
NEPD-3793-2725-EN Birsta 3PH2b, W3, kantbalk A & B h1,2
2 / 8
Product
Product description: Technical data:
Birsta 3P bridge railing has round shapes based on standard profiles to
keep a low cost. The product is
aesthetically pleasing and is therefore used where Market:
it is required a tasteful traffic environment and good transparency, for
example at traffic points, watercourses or cultural places. Sweden
Product specification Reference service life, product
50 years
Materials % Reference service life, building
Steel 95
50 years
Zinc 5
LCA: Calculation rules
Declared unit: Allocation:
The allocation of production data is made in accordance with the provisions
1 m Birsta 3PH2b, W3, kantbalk A & B h1,2
of EN 15804. Incoming energy and water and waste production in-house is
Cut-off criteria: allocated equally among all products through mass allocation. Effects of
primary production of recycled materials is allocated to the main product in
All major raw materials and all the essential energy is included. The
which the material was used. The recycling process and transportation of the
production processes for raw materials and energy flows with very small
material is allocated to this analysis.
amounts (less than 1%) are not included. These cut-off criteria do not
apply for hazardous materials and substances.
Data quality:
Specific data for the product composition are provided by the manufacturer. They represent the production of the declared product and were collected for
EPD development in the year of study. Background data is based on registered EPDs according to EN 15804, Ostfold Research databases, ecoinvent and other
LCA databases. The data quality of the raw materials in A1 is presented in the table below.
Materials Source Data quality Year
Steel Modified ecoinvent 3.5 and 3.6 Database 2020
NEPD-3793-2725-EN Birsta 3PH2b, W3, kantbalk A & B h1,2
3 / 8
System boundary:
Additional technical information:
The product is hot-dip galavanized in accordance with ISO 1461 Na1 Fe/Zn 115 in order to maintain a long service life along the road.
NEPD-3793-2725-EN Birsta 3PH2b, W3, kantbalk A & B h1,2
4 / 8
LCA: Scenarios and additional technical information
The following information describe the scenarios in the different modules of the EPD.
Transport from production place to user (A4)
Capacity utilisation Fuel/Energy
Type Type of vehicle Distance km Unit Value (l/t)
(incl. return) % consumption
Truck 55,0 % Truck, over 32 tonnes, EURO 6 (kgkm) 200 0,022606 l/tkm 4,52
Railway l/tkm
Boat l/tkm
Other Transportation l/tkm
Assembly (A5) End of Life (C1, C3, C4)
. Unit Value . Unit Value
Auxiliary kg Hazardous waste disposed kg
Water consumption m3 Collected as mixed construction waste kg
Electricity consumption kWh Reuse kg
Other energy carriers MJ Recycling kg 50,3712
Material loss kg Energy recovery kg
Output materials from waste treatment kg To landfill kg 0,5088
Dust in the air kg
VOC emissions kg
Transport to waste processing (C2)
Capacity utilisation Fuel/Energy
Type Type of vehicle Distance km Unit Value (l/t)
(incl. return) % consumption
Truck 55,0 % Truck, over 32 tonnes, EURO 6 (kgkm) 200 0,022606 l/tkm 4,52
Railway l/tkm
Boat l/tkm
Other Transportation l/tkm
¨
Benefits and loads beyond the system boundaries (D)
. Unit Value
Substitution of primary steel, with net scrap steel (kg) kg 48,84
NEPD-3793-2725-EN Birsta 3PH2b, W3, kantbalk A & B h1,2
5 / 8
LCA: Results
The LCA results are presented below for the declared unit defined on page 2 of the EPD document.
System boundaries (X=included, MND=module not declared, MNR=module not relevant)
Construction Beyond the
Product stage installation User stage End of life stage . system
stage bondaries
A1 A2 A3 A4 A5 B1 B2 B3 B4 B5 B6 B7 C1 C2 C3 C4 . D
X X X X X MND MND MND MND MND MND MND X X X X . X
Environmental impact
Parameter Unit A1-A3 A4 A5 C1 C2 C3 C4 D
GWP kg CO 2 -eq 5,00E+02 8,82E-01 9,96E-01 9,96E-01 8,82E-01 1,01E-02 2,64E-03 -8,17E+01
ODP kg CFC11 -eq 6,02E-05 1,73E-07 1,80E-07 1,80E-07 1,73E-07 1,11E-09 8,76E-10 -3,37E-06
POCP kg C 2H 4-eq 1,39E-01 1,09E-04 2,00E-04 2,00E-04 1,09E-04 2,76E-06 8,05E-07 -5,70E-02
AP kg SO 2 -eq 3,38E+00 1,85E-03 7,55E-03 7,55E-03 1,85E-03 6,28E-05 1,92E-05 -3,65E-01
EP kg PO 3- -eq 6,67E-01 2,01E-04 1,62E-03 1,62E-03 2,01E-04 9,66E-06 3,39E-06 -1,22E-01
4
ADPM kg Sb -eq 2,40E-02 1,58E-05 3,34E-07 3,34E-07 1,58E-05 7,56E-10 5,10E-11 -1,58E-03
ADPE MJ 6,34E+03 1,44E+01 1,44E+01 1,44E+01 1,44E+01 9,37E-02 7,41E-02 -7,68E+02
GWP Global warming potential; ODP Depletion potential of the stratospheric ozone layer; POCP Formation potential of tropospheric photochemical oxidants;
AP Acidification potential of land and water; EP Eutrophication potential; ADPM Abiotic depletion potential for non fossil resources; ADPE Abiotic depletion
potential for fossil resources
"Reading example: 9,0 E-03 = 9,0*10-3 = 0,009"
*INA Indicator Not Assessed
waR slairetam tropsnarT gnirutcafunaM tropsnarT ylbmessA esU ecnanetniaM riapeR tnemecalpeR tnemhsibrufeR lanoitarepO ygrene esu lanoitarepO esu
retaw
-eD noitcurtsnoc noitilomed tropsnarT etsaW gnissecorp lasopsiD -yrevoceR-esueR -gnilcyceR laitnetop
NEPD-3793-2725-EN Birsta 3PH2b, W3, kantbalk A & B h1,2
6 / 8
Resource use
Parameter Unit A1-A3 A4 A5 C1 C2 C3 C4 D
RPEE MJ 3,25E+02 1,81E-01 8,26E-02 8,26E-02 1,81E-01 7,79E-01 6,05E-04 -6,92E+01
RPEM MJ 3,08E+00 0,00E+00 -3,08E-01 0,00E+00 0,00E+00 0,00E+00 0,00E+00 0,00E+00
TPE MJ 3,28E+02 1,81E-01 8,26E-02 8,26E-02 1,81E-01 7,79E-01 6,05E-04 -6,92E+01
NRPE MJ 6,58E+03 1,45E+01 1,45E+01 1,45E+01 1,45E+01 1,26E-01 7,52E-02 -7,29E+02
NRPM MJ 1,54E+00 0,00E+00 -1,54E-01 0,00E+00 0,00E+00 0,00E+00 0,00E+00 0,00E+00
TRPE MJ 6,58E+03 1,45E+01 1,45E+01 1,45E+01 1,45E+01 1,26E-01 7,52E-02 -7,29E+02
SM kg 1,57E+00 4,97E-03 0,00E+00 0,00E+00 4,97E-03 0,00E+00 0,00E+00 0,00E+00
RSF MJ 1,57E+00 6,33E-03 0,00E+00 0,00E+00 6,33E-03 0,00E+00 0,00E+00 0,00E+00
NRSF MJ 1,65E+00 2,12E-02 0,00E+00 0,00E+00 2,12E-02 0,00E+00 0,00E+00 0,00E+00
W m3 2,05E+02 1,64E-03 1,53E-03 1,53E-03 1,64E-03 5,19E-05 8,14E-05 -4,99E-01
RPEE Renewable primary energy resources used as energy carrier; RPEM Renewable primary energy resources used as raw materials; TPE Total use of renewable
primary energy resources; NRPE Non renewable primary energy resources used as energy carrier; NRPM Non renewable primary energy resources used as
materials; TRPE Total use of non renewable primary energy resources; SM Use of secondary materials; RSF Use of renewable secondary fuels; NRSF Use of non
renewable secondary fuels; W Use of net fresh water
"Reading example: 9,0 E-03 = 9,0*10-3 = 0,009"
*INA Indicator Not Assessed
End of life - Waste
Parameter Unit A1-A3 A4 A5 C1 C2 C3 C4 D
HW kg 1,56E+00 7,88E-04 6,47E-06 6,47E-06 7,88E-04 3,11E-07 1,12E-07 -7,07E-03
NHW kg 2,08E+02 1,25E+00 6,95E-02 6,95E-02 1,25E+00 9,57E-03 5,09E-01 -1,40E+02
RW kg INA* INA* INA* INA* INA* INA* INA* INA*
HW Hazardous waste disposed; NHW Non hazardous waste disposed; RW Radioactive waste disposed
"Reading example: 9,0 E-03 = 9,0*10-3 = 0,009"
*INA Indicator Not Assessed
End of life - Output flow
Parameter Unit A1-A3 A4 A5 C1 C2 C3 C4 D
CR kg 0,00E+00 0,00E+00 0,00E+00 0,00E+00 0,00E+00 0,00E+00 0,00E+00 0,00E+00
MR kg 1,36E-01 6,97E-05 0,00E+00 0,00E+00 6,97E-05 5,04E+01 0,00E+00 0,00E+00
MER kg 2,13E-02 4,30E-03 0,00E+00 0,00E+00 4,30E-03 0,00E+00 0,00E+00 0,00E+00
EEE MJ INA* INA* INA* INA* INA* INA* INA* INA*
ETE MJ INA* INA* INA* INA* INA* INA* INA* INA*
CR Components for reuse; MR Materials for recycling; MER Materials for energy recovery; EEE Exported electric energy; ETE Exported thermal energy
"Reading example: 9,0 E-03 = 9,0*10-3 = 0,009"
*INA Indicator Not Assessed
NEPD-3793-2725-EN Birsta 3PH2b, W3, kantbalk A & B h1,2
7 / 8
Additional Norwegian requirements
Greenhouse gas emissions from the use of electricity in the manufacturing phase
National production mix from import, low voltage (production of transmission lines, in addition to direct emissions and losses in grid) of applied electricity for
the manufacturing process (A3).
Electricity mix Data source Amount Unit
El-mix, Sweden (kWh) ecoinvent 3.4 Alloc Rec 42,67 g CO2-ekv/kWh
Dangerous substances
The product contains no substances given by the REACH Candidate list or the Norwegian priority list.
Indoor environment
Bibliography
ISO 14025:2010 Environmental labels and declarations - Type III environmental declarations - Principles and procedures.
ISO 14044:2006 Environmental management - Life cycle assessment - Requirements and guidelines.
EN 15804:2012+A1:2013 Environmental product declaration - Core rules for the product category of construction products.
ISO 21930:2017 Sustainability in buildings and civil engineering works - Core rules for environmental product declarations of construction products.
ecoinvent v3, Allocation, cut-off by classification, Swiss Centre of Life Cycle Inventories.
Iversen et al., (2018) eEPD v3.0 - Background information for EPD generator system. LCA.no report number 04.18
Vold (2021) EPD generator for Saferoad Background information for customer application and LCA data, LCA.no report number 07.21
NPCR Part A: Construction products and services. Ver. 1.0. April 2017, EPD-Norge.
NPCR 013 Part B for steel and aluminium construction products Ver. 1.0 April 2019, EPD-Norge.
Program operator and publisher Phone: +47 23 08 80 00
The Norwegian EPD Foundation e-mail: post@epd-norge.no
Post Box 5250 Majorstuen, 0303 Oslo,Norway web: www.epd-norge.no
Owner of the declaration Phone: +46 70200648
Saferoad Sverige AB e-mail: ulf.skold@saferoad.se
Volvogatan 2 731 36 Köping web: www.saferoad.se
Author of the Life Cycle Assessment Phone: +47 916 50 916
LCA.no AS e-mail: post@lca.no
Dokka 6B 1671 Kråkerøy web: www.lca.no
Developer of EPD generator Phone: +47 916 50 916
LCA.no AS e-mail: post@lca.no
Dokka 1C,1671 Kråkerøy web: www.lca.no
NEPD-3793-2725-EN Birsta 3PH2b, W3, kantbalk A & B h1,2
8 / 8
