Environmental product declaration
In accordance with 14025 and EN15804+A2
NorDan NTech Villa Balcony door (security) - BE 105/80 (With Aluminium Cladding)
Owner of the declaration: Program operator:
NorDan AS The Norwegian EPD Foundation
Product: Declaration number:
NorDan NTech Villa Balcony door (security) - BE 105/80
(With Aluminium Cladding) Registration number:
Declared unit: Issue date:
1 pcs
Valid to:
This declaration is based on Product Category Rules:
EPD Software:
CEN Standard EN 15804:2012+A2:2019 serves as core
The Norwegian EPD Foundation LCA.no EPD generator ID: 63716
PCR
NCPR 014:2019 Part B for Windows and doors
1 / 14
General information
Product Owner of the declaration:
NorDan NTech Villa Balcony door (security) - BE 105/80 (With NorDan AS
Aluminium Cladding) Contact person: Fredrik Jonsson
Phone: +46 (0) 10-130 01 78
e-mail: fredrik.jonsson@nordan.se
Program operator: Manufacturer:
Post Box 5250 Majorstuen, 0303 Oslo, Norway NorDan AS
The Norwegian EPD Foundation Stasjonsveien 46
Phone: +47 23 08 80 00 4460 Moi, Norway
web: post@epd-norge.no
Declaration number: Place of production:
Egersund NorDan AS
Tengsareidveien 1
4373 Egersund, Norway
This declaration is based on Product Category Rules: Management system:
CEN Standard EN 15804:2012+A2:2019 serves as core PCR NS-ISO 9001:2015, NS-EN ISO 14001:2015
NCPR 014:2019 Part B for Windows and doors
Statement of liability: Organisation no:
The owner of the declaration shall be liable for the underlying 979 776 233
information and evidence. EPD Norway shall not be liable with respect
to manufacturer information, life cycle assessment data and
evidences.​
Declared unit: Issue date:
1 pcs NorDan NTech Villa Balcony door (security) - BE 105/80 (With
Aluminium Cladding)
Declared unit with option: Valid to:
A1-A3,A4,A5,B2,B4,C1,C2,C3,C4,D
Year of study:
2020
Functional unit: Comparability:
1 door set with aluminium cladding measuring 1.23 m x 2.18 m EPD of construction products may not be comparable if they not
(reference door based on EN 14351-1) with an expected service life of comply with EN 15804 and seen in a building context.
60 yrs.
General information on verification of EPD from EPD tools: Development and verification of EPD:
Independent verification of data, other environmental information The declaration is created using EPD tool lca.tools ver EPD2022.03,
and the declaration according to ISO 14025:2010, § 8.1.3 and § 8.1.4. developed by LCA.no. The EPD tool is integrated in the company's
Individualthird party verification of each EPD is not required when the management system, and has been approved by EPD Norway.
EPD tool is i) integrated into the company's environmental
management system, ii) the procedures for use of the EPD tool are Developer of EPD: Linda Jonsson
approved by EPDNorway, and iii)the proccess is reviewed annualy. See
Reviewer of company-specific input data and EPD:​ Jonas Jonsson
Appendix G of EPD-Norway's General Programme Instructions for
further information on EPD tools.
Verification of EPD tool: Approved:
Independent third party verification of the EPD tool, background data
and test-EPD in accordance with EPDNorway's procedures and
guidelines for verification and approval of EPD tools.
Third party verifier:
Gaylord K. Booto, NILU Håkon Hauan, CEO EPD-Norge
(no signature required)
2 / 14
Product
Product description:
Door for use in exterior walls of domestic and commercial buildings.
Product specification
Product NorDan NTech Villa Balcony door (sequrity) - BE in size 1230x2180 mm is covered in this EPD.
Wooden door with aluminium cladding.
Triple glazed unit with tempered glass on the inside/outside 4E# + 16G + 4 + 16G + #E4
Materials kg %
Adhesive and sealant 0,07 0,06
Absorbent - IGU 0,61 0,60
Argon gas - IGU 0,09 0,09
Aluminium 6,49 6,31
Coating materials 1,09 1,05
Glass 59,28 57,58
Gasket 0,43 0,41
Insulation 0,06 0,06
Metal 4,78 4,64
Sealant - IGU 1,40 1,36
Plastic 0,36 0,35
Spacer - IGU 0,72 0,70
Wood 27,57 26,78
Total 102,94
Packaging kg %
Packaging - Plastic 0,10 2,26
Packaging - Cardboard 0,07 1,58
Packaging - Steel 0,06 1,42
Packaging - Wood 4,20 94,74
Total incl. packaging 107,38
Technical data:
Outward opening door. Triple glazed, 105mm frame with 8 mm aluminium clad, 80mm leaf. Uwin 0,85 W/m2K. Certified: BBA - British Board of
Agrément, Secured by Design, NDVK. The total weight of the product is 102,94 kg. The packaging has an average weight of 4,44 kg. Area of
functional unit 2,68 m2. Conversion factor is 0,373 for 1 m2.
Market:
Europe, but scenarios beyond cradle-to-gate are based on the situation in the Norwegian market.
Reference service life, product
The reference service life is 60 years for aluminium cladding timber frame.
Reference service life, building or construction works
60 years
3 / 14
LCA: Calculation rules
Declared unit:
1 pcs NorDan NTech Villa Balcony door (security) - BE 105/80 (With Aluminium Cladding)
Cut-off criteria:
All major raw materials and all the essential energy is included. The production processes for raw materials and energy flows with very small
amounts (less than 1%) are not included. These cut-off criteria do not​ apply for hazardous materials and substances.
Allocation:
The allocation is made in accordance with the provisions of EN 15804. Effects of primary production of recycled materials is allocated to the main
product in which the material was used. The recycling process and transportation of the material is allocated to this analysis. The PCR specific
background data follow the allocation rules in the Ecoinvent v3.7.1 Cut-off database version. The allocation of water, energy and waste flows
within the production facilities for windows and doors follows unit-based allocation adjusted with a point system to different product groups or
products. This score system is regulated by a factor which increases with the resource intensity of each product. The unit-based allocation is
adjusted by the weight of the product, excluding the weight of glass.
Data quality:
Specific data for the product composition are provided by the manufacturer. The data represent the production of the declared product and were
collected for EPD development in the year of study. Background data is based on EPDs according to EN 15804 and different LCA databases. The
data quality of the raw materials in A1 is presented in the table below.
Material quantities of the specified product in reference size have been calculated by NorDan's business system.
The production data was collected in 2021 and is an average for 2020.
Materials Source Data quality Year
Packaging - Cardboard ecoinvent 3.6 Database 2019
Packaging - Plastic ecoinvent 3.6 Database 2019
Packaging - Steel ecoinvent 3.6 Database 2019
Argon gas - IGU ecoinvent 3.7.1 Database 2020
Glass ecoinvent 3.7.1 Database 2020
Insulation ecoinvent 3.7.1 Database 2020
Absorbent - IGU ecoinvent 3.7.1 Specific 2020
Adhesive and sealant ecoinvent 3.7.1 Specific 2020
Aluminium ecoinvent 3.7.1 Specific 2020
Coating materials ecoinvent 3.7.1 Specific 2020
Gasket ecoinvent 3.7.1 Specific 2020
Glass ecoinvent 3.7.1 Specific 2020
Metal ecoinvent 3.7.1 Specific 2020
Plastic ecoinvent 3.7.1 Specific 2020
Sealant - IGU ecoinvent 3.7.1 Specific 2020
Spacer - IGU ecoinvent 3.7.1 Specific 2020
Wood ecoinvent 3.7.1 Specific 2020
Packaging - Wood Modified ecoinvent 3.6 Database 2019
4 / 14
System boundaries (X=included, MND=module not declared, MNR=module not relevant)
Construction Beyond the system
Product stage Use stage End of life stage
installation stage boundaries
A1 A2 A3 A4 A5 B1 B2 B3 B4 B5 B6 B7 C1 C2 C3 C4 D
X X X X X MND X MND X MND MND MND X X X X X
System boundary:
Additional technical information:
For the products with different sizes from the declared unit, the environmental impacts must be converted by using a conversion factor. The
Norwegian EPD Foundation has published instructions on how to interpret EPDs for windows on its website (www.epdnorge.no) where different
calculation methods have been stated. (Document: Bruksanvisninger i hvordan tolke EPD'er - Vinduer).
waR slairetam tropsnarT gnirutcafunaM tropsnarT ylbmessA e​sU ecnanetniaM riapeR tnemecalpeR tnemhsibrufeR lanoitarepO ygrene esu lanoitarepO esu retaw -eD noitcurtsnoc noitilomed tropsnarT etsaW gnissecorp lasopsiD -yrevoceR-esueR laitnetop-gnilcyceR
5 / 14
LCA: Scenarios and additional technical information
The following information describe the scenarios in the different modules of the EPD.
A4
The transport from production to construction site is based on a scenario where the product is transported on a large truck from Egersund to
warehouse in Oslo, Norway (462 km). Transport from warehouse to a construction site is assumed to be 50 km on a medium truck.
A5
According to the report from EPD-Norge Harmonising the documentation of scenarios beyond cradle to gate, EN 15804 there is no loss on site
during construction activities. The product in this EPD is painted and surface treated in the production and not at the building site. Therefore,
there is only 2 items left in this module. 1) Waste treatment of packaging which is considered in the EPD calculations. 1) Energy use during
installation. This can be varied depending on the floor, type of building and several other unknown parameters, and therefore ignored in the
calculation.
B2/B3
The maintenance scenario includes cleaning and painting. Cleaning is performed three times per year. It is calculated with 30 ml of detergent and 3
liters of water each year. Doors with aluminium cladding are assumed to be painted 3 times during its lifetime from the inside. It is assumed that 5
gr of lubricating oil is used every year for fittings and moving parts. The glazing unit is changed once during the lifetime for the doors with
aluminium cladding. No repair is assumed during the product lifetime.
B4/B5
* Number or RSL (Reference Service Life). The door has RSL of 60 years. Therefore, it is assumed to replace the insulated glass unit after 30 years
(See Module B2). The RSL is determined by using SINTEF design guide 700.320. There is no need for refurbishment during the product lifetime.
C1
As there are no data for de-construction, it is assumed no activities in C1 in this study. The product is assumed to be treated as mixed waste and
sent to incineration. The combustible materials are then energy recovered, while glass is assumed to end up in the bottom ash and then landfilled.
The metals are usually sorted out of the bottom ash and then recycled, but there is no data of the share which are recycled and therefore
standard values from Ecoinvent is utilized.
C2
The transport of the product as waste is calculated based on a scenario with 50 km distance.
C3
Doors are assumed to be sorted as mixed construction waste and treated with incineration with energy recovery. However, the manufacturer has
documented the recycling potentials for its product in the Construction Product Declaration eBVD NorDan BE 105 GL Trä/Alu
ID: C-SE556294452901-84
URL: https://ivl-ebvd.azurewebsites.net/BMI/Document/Export/4357/0/Pdf
In the documentation, Chapter 10, the specific material recovery, and energy recovery potential is reported for the product.
C1, C3, C4
The benefits beyond life cycle have been modelled based on the output flows from module C3. This includes energy from incineration and scrap
metal recovered from the ashes. The amount recovered metal is assumed to avoid production of primary metals in accordance to 6.4.3.3 in EN
15804. The exported energy is substituting Norwegian district heating mix and electricity mix. Inventory processes causing substitution of avoided
virgin raw materials has been constructed for each material.
Capacity utilisation Value
Transport from production place to user (A4) Distance (km) Fuel/Energy Consumption Unit
(incl. return) % (Liter/tonne)
Truck, 16-32 tonnes, EURO 6 (kgkm) - RER 36,7 % 50 0,043 l/tkm 2,15
Truck, over 32 tonnes, EURO 6 (kgkm) - RER 53,3 % 462 0,023 l/tkm 10,63
Assembly (A5) Unit Value
Waste, metal, average treatment (kg) kg 0,06
Waste, packaging, folding boxboard, to average
kg 0,07
treatment (kg)
Waste, packaging, pallet, EUR wooden pallet,
kg 4,20
reusable, average treatment (kg) A5
Waste, packaging, plastic film (LDPE), to average
kg 0,10
treatment (kg)
6 / 14
Maintenance (B2) Unit Value
110 Plastic parts, gasket, Ethylene propylene diene
kg/DU 0,43
monomer (EPDM), Europe (kg)
179 Uncoated flat glass, Europe (kg) kg/DU 19,65
186 Glass, coated tempered glass, Europe (kg) kg/DU 39,62
193 Spacer for IGU, Europe (kg) kg/DU 0,72
194 Argon gas for IGU, liquid, global (kg) kg/DU 0,09
208 Sealant for IGU, generic, global (kg) kg/DU 1,40
209 Absorbent for IGU, generic, global (kg) kg/DU 0,61
Detergent, Husvask (kg) kg/DU 1,84
Lubricating oil (kg) - RER kg/DU 0,30
Paint, 40% water, wet mass (kg) kg/DU 0,65
Truck, over 32 tonnes, EURO 5 (kgkm) - RER kgkm/DU 837,00
Waste paint, 40% water, wet mass, incineration in
kg 0,65
Norway (kg)
Waste, glass, incineration (kg) kg 59,28
Waste, metal, average treatment (kg) kg 0,30
Waste, plastic, mixture, for incineration (kg) kg 0,49
Waste, polyurethane, for incineration (kg) kg 2,01
Waste, rubber, unspecified, for incineration (kg) kg 0,43
Water, tap water (kg) - Europe without Switzerland kg/DU 180,00
Capacity utilisation Value
Transport to waste processing (C2) Distance (km) Fuel/Energy Consumption Unit
(incl. return) % (Liter/tonne)
Truck, unspecified (kgkm) - RER 48,7 % 50 0,051 l/tkm 2,55
Waste processing (C3) Unit Value
Materials to recycling (kg) kg 1,95
Waste treatment per kg Glass, incineration with fly
kg 59,37
ash extraction (kg) - CH - C3
Waste treatment per kg Hazardous waste,
kg 0,01
incineration (kg)
Waste treatment per kg municipal solid waste,
kg 0,01
incineration with fly ash extraction (kg)
Waste treatment per kg Paint, hazardous waste
kg 0,92
incineration (kg) - C3
Waste treatment per kg Plastic, Mixture,
kg 0,90
municipal incineration with fly ash extraction (kg)
Waste treatment per kg Polyurethane (PU),
kg 2,79
incineration (kg)
Waste treatment per kg Rubber, municipal
kg 0,43
incineration with fly ash extraction (kg)
Waste treatment per kg Scrap aluminium,
kg 8,40
incineration with fly ash extraction (kg) - CH - C3
Waste treatment per kg Scrap steel, incineration
kg 3,18
with fly ash extraction (kg) - CH - C3
Waste treatment per kg Wood, from incineration
kg 29,69
(kg)
Disposal (C4) Unit Value
Landfilling of ashes from incineration of Glass,
kg 59,37
process of ashes and residues (kg) - CH - C4
Landfilling of ashes from incineration of
kg 0,00
Hazardous waste, from incineration (kg)
Landfilling of ashes from incineration of
Municipal solid waste, process per kg ashes and kg 0,00
residues (kg)
Landfilling of ashes from incineration of Plastics,
Mixture, municipal incineration with fly ash kg 0,03
extraction, process per kg ashes and residues (kg)
Landfilling of ashes from incineration of
Polyurethane (PU), process per kg ashes and kg 0,11
residues - C4 (kg)
Landfilling of ashes from incineration of Rubber,
kg 0,02
process per kg ashes and residues - C4 (kg)
Landfilling of ashes from incineration of Scrap
aluminium, process of ashes and residues (kg) - kg 7,53
CH - C4
Landfilling of ashes from incineration of Scrap
kg 2,10
steel, process of ashes and residues (kg) - CH - C4
Landfilling of ashes from incineration of Wood,
kg 0,34
process per kg ashes and residues - C4 (kg)
Landfilling of ashes from incineration per kg
kg 0,03
Paint, hazardous waste incineration (kg)
7 / 14
Benefits and loads beyond the system
Unit Value
boundaries (D)
Substitution of electricity, in Norway (MJ) MJ 32,65
Substitution of primary aluminium with net scrap
kg 0,52
(kg)
Substitution of primary steel with net scrap (kg) kg 1,66
Substitution of thermal energy, district heating, in
MJ 493,90
Norway (MJ)
8 / 14
LCA: Results
The LCA results are presented below for the declared unit defined on page 2 of the EPD document.
Environmental impact
Indicator Unit A1-A3 A4 A5 B2 B4 C1 C2 C3 C4 D
GWP-total
kg CO2 -
1,53E+02 5,20E+00 6,50E+00 9,47E+01 0 0 7,07E-01 5,98E+01 7,75E-01 -9,52E+00
eq
GWP-fossil
kg CO2 -
2,02E+02 5,20E+00 1,56E-02 9,35E+01 0 0 7,07E-01 1,47E+01 7,75E-01 -9,31E+00
eq
GWP-biogenic
kg CO2 -
-4,92E+01 2,21E-03 6,48E+00 6,90E-01 0 0 3,03E-04 4,51E+01 5,80E-04 -2,82E-02
eq
GWP-luluc
kg CO2 -
2,29E-01 1,63E-03 2,74E-06 5,19E-01 0 0 2,50E-04 4,90E-04 2,34E-04 -1,87E-01
eq
kg
ODP CFC11 - 2,44E-05 1,24E-06 1,82E-09 1,08E-05 0 0 1,61E-07 2,85E-07 2,39E-07 -2,09E-01
eq
mol H+
AP 1,60E+00 1,64E-02 6,42E-05 8,02E-01 0 0 4,03E-03 1,62E-02 5,47E-03 -6,40E-02
-eq
EP-FreshWater kg P -eq 6,95E-03 4,14E-05 1,00E-07 2,11E-03 0 0 5,81E-06 2,32E-05 7,72E-06 -5,45E-04
EP-Marine kg N -eq 2,76E-01 3,55E-03 3,13E-05 1,34E-01 0 0 1,44E-03 7,28E-03 1,95E-03 -1,35E-02
mol N -
EP-Terrestial 3,16E+00 3,96E-02 2,75E-04 1,58E+00 0 0 1,59E-02 7,41E-02 2,15E-02 -1,46E-01
eq
kg
POCP NMVOC 9,06E-01 1,55E-02 7,44E-05 4,07E-01 0 0 4,54E-03 1,90E-02 6,22E-03 -4,68E-02
-eq
ADP- kg Sb -
5,64E-03 1,01E-04 1,86E-07 1,10E-03 0 0 1,83E-05 7,83E-06 1,34E-05 -5,28E-05
minerals&metals1 eq
ADP-fossil1 MJ 2,61E+03 8,34E+01 1,28E-01 1,10E+03 0 0 1,08E+01 2,08E+01 1,77E+01 -1,15E+02
WDP1 m3 4,27E+03 6,66E+01 2,51E-01 1,21E+02 0 0 1,03E+01 7,99E+01 3,50E+01 -3,07E+03
GWP total Global Warming Potential total; GWP fossil Global Warming Potential fossil fuels ; GWP biogenic Global Warming Potential biogenic; GWP luluc Global W
Potential land use change; ODP Ozone Depletion; AP Acidification; EP freshwater Eutrophication aquatic freshwater; EP marine Eutrophication aquatic marine; EP
terrestrial Eutrophication terrestrial ;POCP Photochemical zone formation; ADPE Abiotic Depletion Potential minerals and metals; ADPf Abiotic Depletion Potential fossil
fuels;
"Reading example: 9,0 E-03 = 9,0*10-3 = 0,009"
*INA Indicator Not Assessed
1. The results of this environmental impact indicator shall be used with care as the uncertainties on these results are high or as there is limited experienced with the
indicator
Remarks to environmental impacts
Global warming potential in A1-A3 includes sequestration of carbon in the wood. This amount is accounted as an emission in module C3.
Additionally, it is included sequestration in the wood packaging. This is accounted as an emission in module A5.
9 / 14
Additional environmental impact indicators
Indicator Unit A1-A3 A4 A5 B2 B4 C1 C2 C3 C4 D
PM Disease incidence 1,92E-05 4,51E-07 8,71E-10 8,08E-06 0 0 6,44E-08 2,55E-07 1,00E-07 -1,90E-06
IRP2 kgBq U235 -eq 9,37E+00 3,65E-01 5,15E-04 3,05E+00 0 0 4,74E-02 7,47E-02 7,12E-02 -5,11E-01
ETP-fw1 CTUe 6,84E+03 6,11E+01 1,38E-01 2,89E+03 0 0 8,11E+00 9,67E+01 1,05E+01 -3,94E+02
HTP-c1 CTUh 4,87E-07 0,00E+00 1,00E-11 1,11E-07 0 0 0,00E+00 9,55E-09 3,73E-10 -2,46E-08
HTP-nc1 CTUh 5,37E-06 6,03E-08 4,70E-10 1,12E-06 0 0 1,07E-08 1,05E-07 9,95E-09 -1,59E-07
SQP1 dimensionless 1,26E+04 8,97E+01 1,14E-01 4,63E+02 0 0 9,28E+00 7,50E+00 3,85E+01 -2,75E+02
PM Particulate Matter emissions; IRP Ionizing radiation – human health; ETP-fw Eco toxicity – freshwater; HTP-c Human toxicity – cancer effects; HTP-nc Human
toxicity – non cancer effects; SQP Soil Quality (dimensionless)
"Reading example: 9,0 E-03 = 9,0*10-3 = 0,009"
*INA Indicator Not Assessed
1. The results of this environmental impact indicator shall be used with care as the uncertainties on these results are high or as there is limited experienced with the
indicator
2. This impact category deals mainly with the eventual impact of low dose ionizing radiation on human health of the nuclear fuel cycle. It does not consider effects due
to possible nuclear accidents, occupational exposure nor due to radioactive waste disposal in underground facilities. Potential ionizing radiation from the soil, from
radon and from some construction materials is also not measured by this indicator.
10 / 14
Resource use
Indicator Unit A1-A3 A4 A5 B2 B4 C1 C2 C3 C4 D
PERE MJ 8,30E+02 1,07E+00 2,64E-03 6,44E+01 0 0 1,56E-01 2,92E+00 3,29E-01 -2,75E+02
PERM MJ 5,32E+02 0,00E+00 -6,02E+01 0,00E+00 0 0 0,00E+00 -4,71E+02 0,00E+00 0,00E+00
PERT MJ 1,36E+03 1,07E+00 -4,83E+00 6,44E+01 0 0 1,56E-01 -4,68E+02 3,29E-01 -2,75E+02
PENRE MJ 2,44E+03 8,35E+01 1,28E-01 1,02E+03 0 0 1,08E+01 2,08E+01 1,77E+01 -1,15E+02
PENRM MJ 1,39E+02 0,00E+00 -4,25E+00 0,00E+00 0 0 0,00E+00 -1,34E+02 0,00E+00 0,00E+00
PENRT MJ 2,58E+03 8,35E+01 -4,12E+00 1,02E+03 0 0 1,08E+01 -1,14E+02 1,77E+01 -1,15E+02
SM kg 5,49E-01 0,00E+00 0,00E+00 1,85E-02 0 0 0,00E+00 0,00E+00 0,00E+00 0,00E+00
RSF MJ 1,08E+00 3,77E-02 7,69E-05 4,67E-02 0 0 5,54E-03 6,08E-02 8,71E-03 1,28E-02
NRSF MJ 1,55E+00 1,28E-01 5,70E-04 1,44E-01 0 0 1,95E-02 0,00E+00 3,77E-01 -1,30E+01
FW m3 6,45E+00 9,40E-03 7,45E-05 9,07E-01 0 0 1,23E-03 2,62E-02 1,60E-02 -4,25E-01
PERE Use of renewable primary energy excluding renewable primary energy resources used as raw materials; PERM Use of renewable primary energy resources used as
raw materials; PERT Total use of renewable primary energy resources; PENRE Use of non renewable primary energy excluding non-renewable primary energy resources
used as raw materials; PENRM Use of non renewable primary energy resources used as raw materials; PENRT Total use of non renewable primary energy resources; SM
Use of secondary materials; RSF Use of renewable secondary fuels; NRSF Use of non renewable secondary fuels; FW Use of net fresh water
"Reading example: 9,0 E-03 = 9,0*10-3 = 0,009"
*INA Indicator Not Assessed
11 / 14
End of life - Waste
Indicator Unit A1-A3 A4 A5 B2 B4 C1 C2 C3 C4 D
HWD kg 2,66E+00 4,52E-03 0,00E+00 6,94E+01 0 0 5,85E-04 0,00E+00 6,93E+01 8,11E-03
NHWD kg 5,88E+01 6,75E+00 4,43E-01 1,14E+01 0 0 6,72E-01 5,94E+01 6,37E-01 -3,06E+00
RWD kg 1,05E-02 5,70E-04 0,00E+00 3,76E-03 0 0 7,38E-05 0,00E+00 1,09E-04 -4,50E-04
HWD = Hazardous waste disposed; NHWD = Non-hazardous waste disposed; RWD = Radioactive waste disposed;
"Reading example: 9,0 E-03 = 9,0*10-3 = 0,009"
*INA Indicator Not Assessed
End of life - Output flow
Indicator Unit A1-A3 A4 A5 B2 B4 C1 C2 C3 C4 D
CRU kg 0,00E+00 0,00E+00 0,00E+00 0,00E+00 0 0 0,00E+00 0,00E+00 0,00E+00 0,00E+00
MFR kg 1,98E+00 0,00E+00 2,55E-01 3,30E-01 0 0 0,00E+00 1,95E+00 0,00E+00 0,00E+00
MER kg 4,38E-01 0,00E+00 4,90E-03 1,34E-04 0 0 0,00E+00 1,05E+02 0,00E+00 0,00E+00
EEE MJ 1,74E+00 0,00E+00 9,50E-02 5,34E+00 0 0 0,00E+00 2,77E+01 0,00E+00 0,00E+00
EET MJ 2,56E+01 0,00E+00 1,44E+00 7,77E+01 0 0 0,00E+00 4,19E+02 0,00E+00 0,00E+00
CRU = Components for re-use; MFR = Materials for recycling; MER = Materials for energy recovery; EEE = Exported electrical energy; EET = Exported energy ​ Thermal
"Reading example: 9,0 E-03 = 9,0*10-3 = 0,009"
*INA Indicator Not Assessed
Biogenic Carbon Content
Indicator Unit At the factory gate
Biogenic carbon content in product kg C 1,81E+01
Biogenic carbon content in accompanying packaging kg C 1,77E+00
Note: 1 kg biogenic carbon is equivalent to 44/12 kg CO2
12 / 14
Additional Norwegian requirements
Greenhouse gas emissions from the use of electricity in the manufacturing phase
National production mix from import, low voltage (production of transmission lines, in addition to direct emissions and losses in grid) of applied
electricity for the manufacturing process (A3).
Electricity mix Data source Amount Unit
Electricity, Poland (kWh) ecoinvent 3.6 1060,47 g CO2-eq/kWh
Electricity, Norway (kWh) ecoinvent 3.6 24,33 g CO2-eq/kWh
Dangerous substances
The product contains no substances on the REACH Candidate list or the Norwegian priority list at or above 100 ppm, 0,01 % by weight.
Indoor environment
The product has not been tested for emissions to indoor environments.
Additional Environmental Information
Environmental impact indicators EN 15804+A1 and NPCR Part A v2.0
Indicator Unit A1-A3 A4 A5 B2 B4 C1 C2 C3 C4 D
GWP kg CO2 -eq 5,06E+01 5,15E+00 1,20E-01 1,37E+01 0 0 6,99E-01 5,65E+01 3,06E-02 -9,19E+00
ODP kg CFC11 -eq 3,55E-06 1,00E-06 1,55E-08 6,43E-07 0 0 1,29E-07 6,85E-08 2,44E-09 -7,29E-07
POCP kg C2H4 -eq 7,63E-03 6,35E-04 2,53E-05 2,39E-03 0 0 9,98E-05 1,68E-04 3,45E-06 -6,85E-03
AP kg SO2 -eq 1,62E-01 1,07E-02 5,82E-04 3,57E-02 0 0 1,42E-03 8,09E-03 5,33E-05 -4,95E-02
EP kg PO43- -eq 1,81E-02 1,16E-03 1,73E-04 4,67E-03 0 0 1,48E-04 3,25E-03 7,27E-06 -7,89E-03
ADPM kg Sb -eq 4,17E-04 1,01E-04 1,93E-06 8,41E-05 0 0 1,83E-05 3,21E-06 1,54E-07 -5,28E-05
ADPE MJ 3,69E+02 8,19E+01 1,35E+00 9,96E+01 0 0 1,06E+01 6,37E+00 2,54E-01 -9,86E+01
GWPIOBC kg CO2 -eq 2,16E+02 5,20E+00 8,93E-04 8,65E+01 0 0 7,07E-01 1,14E+01 5,31E-02 -1,02E+01
GWP Global warming potential; ODP Depletion potential of the stratospheric ozone layer; POCP Formation potential of tropospheric photochemical oxidants; AP
Acidification potential of land and water; EP Eutrophication potential; ADPM Abiotic depletion potential for non fossil resources; ADPE Abiotic depletion​ potential for
fossil resources; GWP-IOBC/GHG Global warming potential calculated according to the principle of instantanious oxidation (except emissions and uptake of biogenic
carbon)
13 / 14
Bibliography
ISO 14025:2010 Environmental labels and declarations - Type III environmental declarations - Principles and procedures.
ISO 14044:2006 Environmental management - Life cycle assessment - Requirements and guidelines.
EN 15804:2012+A2:2019 Environmental product declaration - Core rules for the product category of construction products.
ISO 21930:2017 Sustainability in buildings and civil engineering works - Core rules for environmental product declarations of construction
products.
ecoinvent v3, Allocation, cut-off by classification, Swiss Centre of Life Cycle Inventories.
Iversen et al., (2021) eEPD v2021.09 Background information for EPD generator tool system verification, LCA.no Report number: 07.21
Iversen et al., (2022) EPD generator for EPD generator for NPCR 014
Part B for Windows and doors, Background information for EPD generator application and LCA data, LCA.no report number: 17.22
NPCR Part A: Construction products and services. Ver. 2.0. April 2021, EPD-Norge.
NPCR 014 Part B for Windows and doors, Ver. 4.0, 20.09.2021, EPD Norway.
EPD Norway Bruksanvisninger i hvordan tolke EPD'er - Vinduer URL: https://www.epd-norge.no [in Norwegian]
Program operator and publisher Phone: +47 23 08 80 00
The Norwegian EPD Foundation e-mail: post@epd-norge.no
Post Box 5250 Majorstuen, 0303 Oslo, Norway web: www.epd-norge.no
Owner of the declaration: Phone: +46 (0) 10-130 01 78
NorDan AS e-mail: fredrik.jonsson@nordan.se
Stasjonsveien 46, 4460 Moi web: www.nordan.no
Author of the Life Cycle Assessment Phone: +47 98 85 33 33
Norsk Treteknisk Institutt e-mail: firmapost@treteknisk.no
Postboks 113 Blindern, 0314 web: www.treteknisk.no
Developer of EPD generator Phone: +47 916 50 916
LCA.no AS e-mail: post@lca.no
Dokka 6B,1671 Kråkerøy web: www.lca.no
ECO Platform web: www.eco-platform.org
ECO Portal web: ECO Portal
14 / 14
