Environmental product declaration
in accordance with ISO 14025 and EN 15804+A2
NorDan Bor External Door 630G Utsikten Alu (with glass and aluminium cladding)
Owner of the declaration: Program operator:
NorDan AS The Norwegian EPD Foundation
Product: Declaration number:
NorDan Bor External Door 630G Utsikten Alu (with glass
and aluminium cladding) Registration number:
Declared unit: Issue date:
1 pcs
Valid to:
This declaration is based on Product Category Rules:
EPD software:
CEN Standard EN 15804:2012+A2:2019 serves as core
The Norwegian EPD Foundation LCAno EPD generator ID: 217004
PCR
NPCR 014:2019 Part B for Windows and doors
1 / 13
General information
Product Owner of the declaration:
NorDan Bor External Door 630G Utsikten Alu (with glass and NorDan AS
aluminium cladding) Contact person: Fredrik Jonsson
Phone: +46 (0) 10-130 01 78
e-mail: fredrik.jonsson@nordan.se
Program operator: Manufacturer:
Post Box 5250 Majorstuen, 0303 Oslo, Norway NorDan AB
The Norwegian EPD Foundation Grebbestadsvägen 8
Phone: +47 23 08 80 00 457 91 Tanumshede, Sweden
web: post@epd-norge.no
Declaration number: Place of production:
Bor NorDan AB
Kvadervägen
331 74 Bor, Sweden
This declaration is based on Product Category Rules: Management system:
CEN Standard EN 15804:2012+A2:2019 serves as core PCR NS-ISO 9001:2015, NS-EN ISO 14001:2015
NPCR 014:2019 Part B for Windows and doors
Statement of liability: Organisation no:
The owner of the declaration shall be liable for the underlying 979 776 233
information and evidence. EPD Norway shall not be liable with respect
to manufacturer information, life cycle assessment data and
evidences.​
Declared unit: Issue date:
1 pcs NorDan Bor External Door 630G Utsikten Alu (with glass and
aluminium cladding)
Declared unit with option: Valid to:
A1-A3,A4,A5,B2,B4,C1,C2,C3,C4,D
Year of study:
2020
Functional unit: Comparability:
1 pcs external door with glass measuring 1230x2180 mm (reference EPD of construction products may not be comparable if they not
based on EN 14351-1). With expected service life of 30 yrs. comply with EN 15804 and seen in a building context.
General information on verification of EPD from EPD tools: Development and verification of EPD:
Independent verification of data, other environmental information The declaration is created using EPD tool lca.tools ver EPD2022.03,
and the declaration according to ISO 14025:2010, § 8.1.3 and § 8.1.4. developed by LCA.no. The EPD tool is integrated in the company's
Verification of each EPD is made according to EPD-Norway’s management system, and has been approved by EPD Norway.
guidelines for verification and approval requiring that tools are i)
integrated into the company's environmental management system, ii) Developer of EPD: Jonas Jonsson
the procedures for use of the EPD tool are approved by EPD-Norway,
Reviewer of company-specific input data and EPD:​ Linda Jonsson
and iii) the process is reviewed annually by an independent third
party verifier. See Appendix G of EPD-Norway's General Programme
Instructions for further information on EPD tools
Verification of EPD tool: Approved:
Independent third party verification of the EPD tool, background data
and test-EPD in accordance with EPDNorway's procedures and
guidelines for verification and approval of EPD tools. Håkon Hauan, CEO EPD-Norge
Third party verifier:
Gaylord K. Booto, Norwegian Institute for Air Research (NILU)
(no signature required)
2 / 13
Product
Product description:
External door for use in exterior walls of domestic and commercial buildings.
Product specification
Product NorDan Bor external door 630G Utsikten Alu with aluminium cladding in size 1230x2180 mm is covered in this EPD.
Triple glazed unit 4E# + 16G + 4 + 16G + #E4
Materials kg %
Absorbent - IGU 0,58 0,53
Adhesive and sealant 0,29 0,27
Aluminium 11,38 10,48
Argon gas - IGU 0,08 0,07
Coating materials 1,24 1,14
Gasket 0,59 0,55
Glass 51,29 47,23
Medium Density Fibreboard 6,18 5,69
Metal 2,81 2,58
Plastic 0,44 0,40
Sealant - IGU 1,31 1,21
Spacer - IGU 0,68 0,62
Wood 31,73 29,22
Total 108,60
Packaging kg %
Packaging - Cardboard 5,15 53,73
Packaging - Plastic 0,17 1,78
Packaging - Steel 0,06 0,66
Packaging - Wood 4,20 43,83
Total incl. packaging 118,18
Technical data:
External door with 10mm aluminium cladding. Triple glazed, 115 mm frame with 79 mm door leaf. U-value 1,0 W/m2K. The total weight of the
product is 108,6 kg and the packaging has an average weight of 9,58 kg.
Area of functional unit 2,68m2. Conversion factor is 0,373 for 1 m2
Market:
Europe, but scenarios beyond cradle-to-gate are based on the situation in the Norwegian market.
Reference service life, product
The reference service life is 30 years for doors.
Reference service life, building or construction works
60 years
3 / 13
LCA: Calculation rules
Declared unit:
1 pcs NorDan Bor External Door 630G Utsikten Alu (with glass and aluminium cladding)
Cut-off criteria:
All major raw materials and all the essential energy is included. The production processes for raw materials and energy flows with very small
amounts (less than 1%) are not included. These cut-off criteria do not​ apply for hazardous materials and substances.
Allocation:
The allocation is made in accordance with the provisions of EN 15804. Effects of primary production of recycled materials is allocated to the main
product in which the material was used. The recycling process and transportation of the material is allocated to this analysis. The PCR specific
background data follow the allocation rules in the Ecoinvent v3.7.1 Cut-off database version. The allocation of water, energy and waste flows
within the production facilities for windows and doors follows unit-based allocation adjusted with a point system to different product groups or
products. This score system is regulated by a factor which increases with the resource intensity of each product. The unit-based allocation is
adjusted by the weight of the product, excluding the weight of glass.
Data quality:
Specific data for the product composition are provided by the manufacturer. The data represent the production of the declared product and were
collected for EPD development in the year of study. Background data is based on EPDs according to EN 15804 and different LCA databases. The
data quality of the raw materials in A1 is presented in the table below.
Material quantities of the specified product in reference size have been calculated by NorDan's business system. The production data was collected
in 2021 and is an average for 2020.
Materials Source Data quality Year
Absorbent - IGU ecoinvent 3.7.1 Specific 2020
Adhesive and sealant ecoinvent 3.7.1 Specific 2020
Aluminium ecoinvent 3.7.1 Specific 2020
Argon gas - IGU ecoinvent 3.7.1 Database 2020
Coating materials ecoinvent 3.7.1 Specific 2020
Gasket ecoinvent 3.7.1 Specific 2020
Glass ecoinvent 3.7.1 Database 2020
Glass ecoinvent 3.7.1 Specific 2020
Medium Density Fibreboard ecoinvent 3.7.1 Specific 2020
Metal ecoinvent 3.7.1 Specific 2020
Packaging - Cardboard ecoinvent 3.6 Database 2019
Packaging - Plastic ecoinvent 3.6 Database 2019
Packaging - Steel ecoinvent 3.6 Database 2019
Packaging - Wood Modified ecoinvent 3.6 Database 2019
Plastic ecoinvent 3.7.1 Specific 2020
Sealant - IGU ecoinvent 3.7.1 Specific 2020
Spacer - IGU ecoinvent 3.7.1 Specific 2020
Wood ecoinvent 3.7.1 Specific 2020
4 / 13
System boundaries (X=included, MND=module not declared, MNR=module not relevant)
Construction Beyond the system
Product stage Use stage End of life stage
installation stage boundaries
A1 A2 A3 A4 A5 B1 B2 B3 B4 B5 B6 B7 C1 C2 C3 C4 D
X X X X X MND X MND X MND MND MND X X X X X
System boundary:
Additional technical information:
For the products with different sizes from the declared unit, the environmental impacts must be converted by using a conversion factor. The
Norwegian EPD Foundation has published instructions on how to interpret EPDs for windows on its website (www.epdnorge.no) where different
calculation methods have been stated. (Document: Bruksanvisninger i hvordan tolke EPD'er - Vinduer).
waR slairetam tropsnarT gnirutcafunaM tropsnarT ylbmessA e​sU ecnanetniaM riapeR tnemecalpeR tnemhsibrufeR lanoitarepO ygrene esu lanoitarepO esu retaw -eD noitcurtsnoc noitilomed tropsnarT etsaW gnissecorp lasopsiD -yrevoceR-esueR laitnetop-gnilcyceR
5 / 13
LCA: Scenarios and additional technical information
The following information describe the scenarios in the different modules of the EPD.
A4
The transportation from production to construction site is based on a scenario where the product is transported from factory to terminal is
assumed to be 75 km on a medium truck. Transport from terminal to warehouse in Oslo, Norway on a large lorry (439 km). Transport from
warehouse to a construction site is assumed to be 50 km on a medium truck.
A5
According to the report from EPD-Norge Harmonising the documentation of scenarios beyond cradle to gate, EN 15804 there is no loss on site
during construction activities. The product in this EPD is painted and surface treated in the production and not at the building site. Therefore,
there is only 2 items left in this module. 1) Waste treatment of packaging which is considered in the EPD calculations. 1) Energy use during
installation. This can be varied depending on the floor, type of building and several other unknown parameters, and therefore ignored in the
calculation.
B2/B3
The maintenance scenario includes cleaning and painting. Cleaning is performed two times per year. It is calculated with 30 ml of detergent and 3
liters of water each year. Doors are assumed to be painted 1 time during its lifetime from inside, due to aluminum cladding, the outside does not
need to be repainted. It is assumed that 5 gr of lubricating oil is used every year for fittings and moving parts. No repair is assumed during the
product lifetime.
B4/B5
* Number or RSL (Reference Service Life). Door with 30 years RSL is assumed to have one entire door replacement during the lifetime of the
building. It is assumed that this change is occurred after 30 years when the IGU reaches its end of life. There is no need for refurbishment during
the product lifetime.
C1
As there are no data for de-construction, it is assumed no activities in C1 in this study. The door is assumed to be treated as mixed waste and sent
to incineration. The combustible materials are then energy recovered, while glass is assumed to end up in the bottom ash and then landfilled. The
metals are usually sorted out of the bottom ash and then recycled, but there is no data of the share which are recycled and therefore standard
values from Ecoinvent is utilized.
C2
The transport of the product as waste is calculated based on a scenario with 50 km distance.
C3
Doors are assumed to be sorted as mixed construction waste and treated with incineration with energy recovery. However, the manufacturer has
documented the recycling potentials for its product in the BPD (Building Product Declaration).
BPD is published on NorDan's public document system, NDocs.
Name: BPD_NorDan Bor External Door 630G Utsikten Alu (with glass and aluminium cladding)
URL: https://portal.nordan.no/ndocs/search?category=document_EPD
In the documentation, Chapter 10, the specific material recovery, and energy recovery potential is reported for the product.
C1, C3, C4
The benefits beyond life cycle have been modelled based on the output flows from module C3. This includes energy from incineration and scrap
metal recovered from the ashes. The amount recovered metal is assumed to avoid production of primary metals in accordance to 6.4.3.3 in EN
15804. The exported energy is substituting Norwegian district heating mix and electricity mix. Inventory processes causing substitution of avoided
virgin raw materials has been constructed for each material.
Capacity utilisation Value
Transport from production place to user (A4) Distance (km) Fuel/Energy Consumption Unit
(incl. return) % (Liter/tonne)
Truck, 16-32 tonnes, EURO 6 (kgkm) - RER 36,7 % 125 0,043 l/tkm 5,38
Truck, over 32 tonnes, EURO 6 (kgkm) - RER 53,3 % 439 0,023 l/tkm 10,10
Assembly (A5) Unit Value
Waste, metal, average treatment (kg) kg 0,06
Waste, packaging, folding boxboard, to average
kg 5,15
treatment (kg)
Waste, packaging, pallet, EUR wooden pallet,
kg 4,20
reusable, average treatment (kg) A5
Waste, packaging, PET straps, 0% recycled, to
kg 0,07
average treatment (kg)
Waste, packaging, plastic film (LDPE), to average
kg 0,10
treatment (kg)
6 / 13
Maintenance (B2) Unit Value
Detergent, Husvask (kg) kg/DU 1,84
Lubricating oil (kg) - RER kg/DU 0,30
Paint, 40% water, wet mass (kg) kg/DU 0,30
Truck, unspecified (kgkm) - RER kgkm/DU 732,00
Waste paint, 40% water, wet mass, incineration in
Norway (kg) kg 0,30
Water, tap water (kg) - Europe without Switzerland kg/DU 180,00
Replacement (B4) Unit Value
Replacement (p) Units/DU 1,00
Waste treatment of replaced materials (p) Units 1,00
Capacity utilisation Value
Transport to waste processing (C2) Distance (km) Fuel/Energy Consumption Unit
(incl. return) % (Liter/tonne)
Truck, unspecified (kgkm) - RER 48,7 % 50 0,051 l/tkm 2,55
Waste processing (C3) Unit Value
Materials to recycling (kg) kg 1,99
Waste treatment per kg Glass, incineration with fly
kg 51,37
ash extraction (kg) - CH - C3
Waste treatment per kg Hazardous waste,
kg 0,00
incineration (kg)
Waste treatment per kg municipal solid waste,
kg 0,01
incineration with fly ash extraction (kg)
Waste treatment per kg Paint, hazardous waste
kg 1,23
incineration (kg) - C3
Waste treatment per kg Plastic, Mixture,
kg 0,98
municipal incineration with fly ash extraction (kg)
Waste treatment per kg Polyurethane (PU),
kg 3,12
incineration (kg)
Waste treatment per kg Rubber, municipal
kg 0,59
incineration with fly ash extraction (kg)
Waste treatment per kg Scrap aluminium,
kg 12,38
incineration with fly ash extraction (kg) - CH - C3
Waste treatment per kg Scrap steel, incineration
kg 2,09
with fly ash extraction (kg) - CH - C3
Waste treatment per kg Wood, from incineration
kg 40,93
(kg)
Disposal (C4) Unit Value
Landfilling of ashes from incineration of Glass,
kg 51,37
process of ashes and residues (kg) - CH - C4
Landfilling of ashes from incineration of
kg 0,00
Hazardous waste, from incineration (kg)
Landfilling of ashes from incineration of
Municipal solid waste, process per kg ashes and kg 0,00
residues (kg)
Landfilling of ashes from incineration of Plastics,
Mixture, municipal incineration with fly ash kg 0,03
extraction, process per kg ashes and residues (kg)
Landfilling of ashes from incineration of
Polyurethane (PU), process per kg ashes and kg 0,12
residues - C4 (kg)
Landfilling of ashes from incineration of Rubber,
kg 0,03
process per kg ashes and residues - C4 (kg)
Landfilling of ashes from incineration of Scrap
aluminium, process of ashes and residues (kg) - kg 11,09
CH - C4
Landfilling of ashes from incineration of Scrap
kg 1,38
steel, process of ashes and residues (kg) - CH - C4
Landfilling of ashes from incineration of Wood,
kg 0,47
process per kg ashes and residues - C4 (kg)
Landfilling of ashes from incineration per kg
kg 0,04
Paint, hazardous waste incineration (kg)
Benefits and loads beyond the system
Unit Value
boundaries (D)
Substitution of electricity, in Norway (MJ) MJ 35,85
Substitution of primary aluminium with net scrap
kg 0,89
(kg)
Substitution of primary steel with net scrap (kg) kg 0,71
Substitution of thermal energy, district heating, in
MJ 542,42
Norway (MJ)
7 / 13
LCA: Results
The LCA results are presented below for the declared unit defined on page 2 of the EPD document.
Environmental impact
Indicator Unit A1-A3 A4 A5 B2 B4 C1 C2 C3 C4 D
GWP-total
kg CO2 -
1,77E+02 6,94E+00 1,51E+01 3,37E+00 1,99E+02 0 7,78E-01 7,96E+01 7,30E-01 -1,21E+01
eq
GWP-fossil
kg CO2 -
2,50E+02 6,93E+00 1,03E-01 3,12E+00 2,57E+02 0 7,78E-01 1,74E+01 7,29E-01 -1,18E+01
eq
GWP-biogenic
kg CO2 -
-7,40E+01 2,93E-03 1,50E+01 9,95E-03 -5,90E+01 0 3,34E-04 6,22E+01 5,43E-04 -4,31E-02
eq
GWP-luluc
kg CO2 -
8,57E-01 2,24E-03 3,03E-05 2,41E-01 8,60E-01 0 2,75E-04 6,05E-04 2,18E-04 -2,58E-01
eq
kg
ODP CFC11 - 3,12E-05 1,64E-06 1,95E-08 3,89E-07 3,28E-05 0 1,77E-07 3,62E-07 2,23E-07 -2,29E-01
eq
mol H+
AP 1,84E+00 2,15E-02 4,60E-04 2,16E-02 1,87E+00 0 4,43E-03 2,00E-02 5,10E-03 -8,30E-02
-eq
EP-FreshWater kg P -eq 9,43E-03 5,52E-05 7,86E-07 1,58E-04 9,48E-03 0 6,40E-06 2,66E-05 7,32E-06 -6,32E-04
EP-Marine kg N -eq 3,29E-01 4,56E-03 1,66E-04 3,31E-03 3,34E-01 0 1,59E-03 8,90E-03 1,82E-03 -1,60E-02
mol N -
EP-Terrestial 3,75E+00 5,09E-02 1,69E-03 3,01E-02 3,80E+00 0 1,75E-02 9,11E-02 2,01E-02 -1,74E-01
eq
kg
POCP NMVOC 1,11E+00 1,98E-02 4,83E-04 1,84E-02 1,13E+00 0 4,99E-03 2,33E-02 5,79E-03 -5,41E-02
-eq
ADP- kg Sb-
3,86E-03 1,47E-04 2,21E-06 6,05E-05 4,01E-03 0 2,01E-05 9,32E-06 1,24E-05 -3,27E-05
minerals&metals1 eq
ADP-fossil1 MJ 3,74E+03 1,10E+02 1,30E+00 7,06E+01 3,85E+03 0 1,19E+01 2,60E+01 1,65E+01 -1,52E+02
WDP1 m3 6,29E+04 9,16E+01 1,79E+00 4,61E+01 6,30E+04 0 1,13E+01 9,99E+01 3,36E+01 -5,03E+03
GWP-total = Global Warming Potential total; GWP-fossil = Global Warming Potential fossil fuels; GWP-biogenic = Global Warming Potential biogenic; GWP-luluc =
Global Warming Potential land use and land use change; ODP = Depletion potential of the stratospheric ozone layer; AP = Acidification potential, Accumulated
Exceedance; EP-freshwater = Eutrophication potential, fraction of nutrients reaching freshwater end compartment: EP-marine = Eutrophication potential, fraction of
nutrients reaching marine end compartment; EP-terrestrial = Eutrophication potential, Accumulated Exceedance; POCP = Formation potential of tropospheric ozone;
ADP-minerals&metals = Abiotic depletion potential for non-fossil resources; ADP-fossil = Abiotic depletion for fossil resources potential; WDP = Water (user)
deprivation potential, deprivation-weighted water consumption
"Reading example: 9,0 E-03 = 9,0*10-3 = 0,009"
*INA Indicator Not Assessed
1. The results of this environmental impact indicator shall be used with care as the uncertainties on these results are high or as there is limited experienced with the
indicator
Remarks to environmental impacts
Global warming potential in A1-A3 includes sequestration of carbon in the wood. This amount is accounted as an emission in module C3.
Additionally, it is included sequestration in the wood packaging. This is accounted as an emission in module A5.
8 / 13
Additional environmental impact indicators
Indicator Unit A1-A3 A4 A5 B2 B4 C1 C2 C3 C4 D
PM Disease incidence 2,77E-05 5,63E-07 6,74E-09 1,38E-07 2,83E-05 0 7,09E-08 2,88E-07 9,31E-08 -2,18E-06
IRP2 kgBq U235 -eq 3,19E+01 4,80E-01 5,54E-03 1,64E-01 3,24E+01 0 5,22E-02 9,51E-02 6,63E-02 -7,20E-01
ETP-fw1 CTUe 7,94E+03 8,07E+01 1,69E+00 6,66E+01 8,03E+03 0 8,93E+00 1,25E+02 9,88E+00 -4,07E+02
HTP-c1 CTUh 6,63E-07 0,00E+00 5,60E-11 4,07E-09 6,63E-07 0 0,00E+00 1,21E-08 3,58E-10 -2,81E-08
HTP-nc1 CTUh 7,02E-06 8,14E-08 2,42E-09 4,52E-08 7,11E-06 0 1,18E-08 1,31E-07 9,61E-09 -3,85E-07
SQP1 dimensionless 1,57E+04 1,10E+02 9,26E-01 2,68E+01 1,58E+04 0 1,02E+01 9,64E+00 3,60E+01 -3,02E+02
PM = Particulate Matter emissions; IRP = Ionizing radiation – human health; ETP-fw = Eco toxicity – freshwater; HTP-c = Human toxicity – cancer effects; HTP-nc =
Human toxicity – non cancer effects; SQP = Potential Soil Quality Index (dimensionless)
"Reading example: 9,0 E-03 = 9,0*10-3 = 0,009"
*INA Indicator Not Assessed
1. The results of this environmental impact indicator shall be used with care as the uncertainties on these results are high or as there is limited experienced with the
indicator
2. This impact category deals mainly with the eventual impact of low dose ionizing radiation on human health of the nuclear fuel cycle. It does not consider effects due
to possible nuclear accidents, occupational exposure nor due to radioactive waste disposal in underground facilities. Potential ionizing radiation from the soil, from
radon and from some construction materials is also not measured by this indicator.
9 / 13
Resource use
Indicator Unit A1-A3 A4 A5 B2 B4 C1 C2 C3 C4 D
PERE MJ 1,93E+03 1,45E+00 2,21E-02 5,17E+00 1,93E+03 0 1,71E-01 3,82E+00 3,11E-01 -3,15E+02
PERM MJ 8,49E+02 0,00E+00 -1,99E+02 0,00E+00 6,50E+02 0 0,00E+00 -6,49E+02 0,00E+00 0,00E+00
PERT MJ 2,77E+03 1,45E+00 -1,99E+02 5,17E+00 2,58E+03 0 1,71E-01 -6,45E+02 3,11E-01 -3,15E+02
PENRE MJ 3,57E+03 1,10E+02 1,30E+00 7,10E+01 3,68E+03 0 1,19E+01 2,60E+01 1,65E+01 -1,52E+02
PENRM MJ 1,47E+02 0,00E+00 -5,88E+00 0,00E+00 1,41E+02 0 0,00E+00 -1,55E+02 0,00E+00 0,00E+00
PENRT MJ 3,71E+03 1,10E+02 -4,58E+00 7,10E+01 3,82E+03 0 1,19E+01 -1,29E+02 1,65E+01 -1,52E+02
SM kg 1,12E+00 0,00E+00 0,00E+00 0,00E+00 1,12E+00 0 0,00E+00 0,00E+00 0,00E+00 0,00E+00
RSF MJ 3,89E+00 5,10E-02 7,20E-04 3,44E-02 3,95E+00 0 6,10E-03 7,95E-02 8,23E-03 -3,52E-02
NRSF MJ 5,29E+00 1,75E-01 3,20E-03 1,46E-02 5,46E+00 0 2,14E-02 0,00E+00 4,08E-01 -1,56E+01
FW m3 8,30E+00 1,23E-02 6,29E-04 2,30E-01 8,32E+00 0 1,35E-03 3,10E-02 1,49E-02 -5,34E-01
PERE = Use of renewable primary energy excluding renewable primary energy resources used as raw materials; PERM = Use of renewable primary energy resources used
as raw materials; PERT = Total use of renewable primary energy resources; PENRE = Use of non renewable primary energy excluding non-renewable primary energy
resources used as raw materials; PENRM = Use of non renewable primary energy resources used as raw materials; PENRT = Total use of non renewable primary energy
resources; SM = Use of secondary materials; RSF = Use of renewable secondary fuels; NRSF = Use of non-renewable secondary fuels; FW = Net use of fresh water
"Reading example: 9,0 E-03 = 9,0*10-3 = 0,009"
*INA Indicator Not Assessed
10 / 13
End of life - Waste
Indicator Unit A1-A3 A4 A5 B2 B4 C1 C2 C3 C4 D
HWD kg 4,62E+00 5,90E-03 0,00E+00 1,50E-02 4,63E+00 0 6,44E-04 0,00E+00 6,42E+01 2,70E-02
NHWD kg 7,02E+01 8,15E+00 5,59E+00 6,93E-01 8,40E+01 0 7,40E-01 5,14E+01 6,79E-01 -3,67E+00
RWD kg 2,15E-02 7,50E-04 0,00E+00 1,98E-04 2,23E-02 0 8,12E-05 0,00E+00 1,01E-04 -6,42E-04
HWD = Hazardous waste disposed; NHWD = Non-hazardous waste disposed; RWD = Radioactive waste disposed
"Reading example: 9,0 E-03 = 9,0*10-3 = 0,009"
*INA Indicator Not Assessed
End of life - Output flow
Indicator Unit A1-A3 A4 A5 B2 B4 C1 C2 C3 C4 D
CRU kg 0,00E+00 0,00E+00 3,99E+00 0,00E+00 3,99E+00 0 0,00E+00 0,00E+00 0,00E+00 0,00E+00
MFR kg 5,39E+00 0,00E+00 4,94E+00 0,00E+00 1,03E+01 0 0,00E+00 1,99E+00 0,00E+00 0,00E+00
MER kg 6,48E+00 0,00E+00 5,68E-01 0,00E+00 7,05E+00 0 0,00E+00 1,11E+02 0,00E+00 0,00E+00
EEE MJ 4,41E+00 0,00E+00 4,39E-01 1,77E-01 4,85E+00 0 0,00E+00 3,63E+01 0,00E+00 0,00E+00
EET MJ 5,54E+01 0,00E+00 6,65E+00 1,23E+00 6,20E+01 0 0,00E+00 5,50E+02 0,00E+00 0,00E+00
CRU = Components for re-use; MFR = Materials for recycling; MER = Materials for energy recovery; EEE = Exported energy electrical; EET = Exported energy thermal
"Reading example: 9,0 E-03 = 9,0*10-3 = 0,009"
*INA Indicator Not Assessed
Biogenic Carbon Content
Indicator Unit At the factory gate
Biogenic carbon content in product kg C 2,28E+01
Biogenic carbon content in accompanying packaging kg C 4,10E+00
Note: 1 kg biogenic carbon is equivalent to 44/12 kg CO2
11 / 13
Additional requirements
Greenhouse gas emissions from the use of electricity in the manufacturing phase
National production mix from import, low voltage (production of transmission lines, in addition to direct emissions and losses in grid) of applied
electricity for the manufacturing process (A3).
Electricity mix Data source Amount Unit
Electricity, Poland (kWh) ecoinvent 3.6 1060,47 g CO2-eq/kWh
Electricity, Sweden (kWh) ecoinvent 3.6 54,94 g CO2-eq/kWh
Dangerous substances
The product contains substances given by the REACH Candidate list that are less than 0,1 % by weight.
Indoor environment
The product has not been tested for emissions to indoor environments.
Additional Environmental Information
Additional environmental impact indicators required in NPCR Part A for construction products
Indicator Unit A1-A3 A4 A5 B2 B4 C1 C2 C3 C4 D
GWPIOBC kg CO2 -eq 2,73E+02 6,94E+00 1,03E-01 3,37E+00 2,80E+02 0 7,78E-01 1,74E+01 7,33E-01 -1,21E+01
GWP-IOBC: Global warming potential calculated according to the principle of instantaneous oxidation. In order to increase the transparency of biogenic carbon​
contribution to climate impact, the indicator GWP-IOBC is required as it declares climate impacts calculated according to the principle of instantaneous oxidation.​
GWP-IOBC is also referred to as GWP-GHG in context to Swedish public procurement legislation.
12 / 13
Bibliography
ISO 14025:2010 Environmental labels and declarations - Type III environmental declarations - Principles and procedures.
ISO 14044:2006 Environmental management - Life cycle assessment - Requirements and guidelines.
EN 15804:2012+A2:2019 Environmental product declaration - Core rules for the product category of construction products.
ISO 21930:2017 Sustainability in buildings and civil engineering works - Core rules for environmental product declarations of construction
products.
ecoinvent v3, Allocation, cut-off by classification, Swiss Centre of Life Cycle Inventories.
Iversen et al., (2021) eEPD v2021.09 Background information for EPD generator tool system verification, LCA.no Report number: 07.21
Iversen et al., (2022) EPD generator for EPD generator for NPCR 014
Part B for Windows and doors, Background information for EPD generator application and LCA data, LCA.no report number: 17.22
NPCR Part A: Construction products and services. Ver. 2.0. April 2021, EPD-Norge.
NPCR 014 Part B for Windows and doors, Ver. 4.0, 20.09.2021, EPD Norway.
EPD Norway Bruksanvisninger i hvordan tolke EPD'er - Vinduer URL: https://www.epd-norge.no [in Norwegian]
Program operator and publisher Phone: +47 23 08 80 00
The Norwegian EPD Foundation e-mail: post@epd-norge.no
Post Box 5250 Majorstuen, 0303 Oslo, Norway web: www.epd-norge.no
Owner of the declaration: Phone: +46 (0) 10-130 01 78
NorDan AS e-mail: fredrik.jonsson@nordan.se
Stasjonsveien 46, 4460 Moi web: www.nordan.no
Author of the Life Cycle Assessment Phone: +47 98 85 33 33
Norsk Treteknisk Institutt e-mail: firmapost@treteknisk.no
Postboks 113 Blindern, 0314 web: www.treteknisk.no
Developer of EPD generator Phone: +47 916 50 916
LCA.no AS e-mail: post@lca.no
Dokka 6B,1671 Kråkerøy web: www.lca.no
ECO Platform web: www.eco-platform.org
ECO Portal web: ECO Portal
13 / 13
