ver1 2015
ENVIRONMENTAL PRODUCT DECLARATION
in accordance with ISO 14025, ISO 21930 and EN 15804
Owner of the declaration: Flokk Holding A S - O FFEC C T
Program operator: The Norwegian EP D Foundation
Publisher: The Norwegian EP D Foundation
Declaration number: NEPD-2268-1031-EN
Registration number: NEPD-2268-1031-EN
ECO Platform reference number: -
Issue date: 17.06.2020
Valid to: 17.06.2025
OFFECCT Carry On
Flokk Holding AS - OFFECCT
www.epd-norge.no
NEPD-2268-1031-EN OFFECCT Carry On 1 / 8
General information
Product: Owner of the declaration:
OFFECCT Carry On Flokk Holding AS - OFFECCT
Contact person: Helena Lidenfors
Åberg
Phone:
e-mail: helena.l.aberg@offecct.se
Program operator: Manufacturer:
Flokk Holding AS - OFFECCT
The Norwegian EP D Foundation
P b. 5250 Majorstuen, 0303 O slo
P hone: +47 23 08 80 00
e-mail: post@epd-norge.no
Declaration number: Place of production:
OFFECCT Grönhultsvägen, Tibro. Sweden
NEPD-2268-1031-EN
ECO Platform reference number: Management system:
ISO 14001, Certificate No. 14001-0336 ISO 9001, Certificate
No.9001-0336 From the accredited unit: SCAB Svensk
Certifiering Norden AB
This declaration is based on Product Category Rules: Organisation no:
No 925 902 749
CEN Standard EN 15804:2012+A1:2013 serves as core PCR
Statement of liability: Issue date: 17.06.2020
The owner of the declaration shall be liable for the underlying
information and evidence. EPD Norway shall not be liable with
respect to manufacturer information, life cycle assessment data Valid to: 17.06.2025
and evidences.
Declared unit: Year of study:
1 Pcs OFFECCT Carry On 2020
Declared unit with option: Comparability:
A1,A2,A3,A4,A5,C1,C2,C3,D EPDs from programmes other than the Norwegian EPD
Foundation may not be comparable
Functional unit: Author of the Life Cycle Assessment:
The declaration is developed using eEPD v4.0 from LCA.no
Approval:
Company specific data are:
Collected/registered by: Helena Lidenfors Åberg
Internal verification by: Laura Fouilland
Verification: Approved:
Independent verification of data, other environmental information
and the declaration according to ISO14025:2010, § 8.1.3 and §
8.1.4
Third party verifier:
Sign
Sign
Seniorforsker Erik Svanes
(Independent verifier approved by EPD Norway)
Key environmental indicators Unit Cradle to gate A1 - A3
Global warming kg CO2 eqv 23,70
Total energy use MJ 503,71
Amount of recycled materials % 22,85
NEPD-2268-1031-EN OFFECCT Carry On 2 / 8
Product
Market: Technical data:
Frame in wood with cold foam.
Worldwide
Upholstered in fabric (for EPD Re-wool from Kvadrat AS is used).
Product description: High compressed handle in white pigmented ash, casted fitting in
zinc.
Carry On is a portable seating solution that works perfectly by itself
but also as a complement to other products. Carry On is designed Reference service life, product
by Mattias Stenberg who has a strong belief in the need of flexible
working places in the public space.Today we work more in projects 15 years - can be prolonged if reupholstered
and need environments that can be easily adapted to different
Reference service life, building
needs. Carry On is not only physically flexible, it also signals to the
user how it should be used by the handle on top. Carry On has round
but simple forms and combines traditional materials and
craftsmanship with contemporary design and functions. It gives a
tailored impression with stitching that communicates good
craftsmanship. It is easy to stack Carry On, which means that it
does not
have to be stored elsewhere when not used.
Product specification
H 450/560, S 455, W 450/490, Ø450
Recycled share in Recycled share in
Materials kg %
material (kg) material (%)
Metal - Steel 0,47 8,32 0,24 50,00
Metal - Zinc 0,10 1,77 0,00 0,00
Textile - Wool 0,45 7,96 0,45 100,00
Plastic - Polyurethane (PUR) 1,90 33,63 0,00 0,00
Plastic - Polypropylene (PP) 0,20 3,54 0,10 50,00
Rubber, synthetic 0,02 0,35 0,00 0,00
Wood - Plywood 1,60 28,32 0,00 0,00
Wood - Solid spruce 0,60 10,62 0,00 0,00
Glue for wood 0,01 0,18 0,00 0,00
Plastic - Polyethylene (HDPE) 0,30 5,31 0,00 0,00
Recycled share in Recycled share in
Packaging kg
material (kg) material (%)
Packaging - Cardboard 1,00 0,76 76,30
Packaging - Plastic 0,01 0,00 0,00
Packaging - Paper 0,20 0,00 0,00
LCA: Calculation rules
Declared unit: Allocation:
The allocation is made in accordance with the provisions of EN
1 Pcs OFFECCT Carry On
15804. Effects of primary production of recycled materials is
Cut-off criteria: allocated to the main product in which the material was used. The
recycling process and transportation of the material is allocated to
All major raw materials and all the essential energy is included. The
this analysis.
production processes for raw materials and energy flows with very
small amounts (less than 1%) are not included. These cut-off Where virgin materials are used, emissions and energy consumption
criteria do not apply for hazardous materials and substances. connected with extraction and production
are included. Where recycled materials are used in the product,
emissions and energy consumption related to the recycling
process are included. Emissions from incineration are allocated to
the product system that uses the recovered energy.
Data quality:
Specific data for the product composition are provided by the manufacturer. They represent the production of the declared product and were
collected for EPD development in the year of study. Background data is based on registered EPDs according to EN 15804, Ostfold
Research databases, ecoinvent and other LCA databases. The data quality of the raw materials in A1 is presented in the table below.
Specific manufacturing data from 2019 are used. Data from Ecoinvent 3.4 and Østfoldforskning databases are used as the basis for raw
materials and energy carrier production.
NEPD-2268-1031-EN OFFECCT Carry On 3 / 8
System boundary:
Life cycle stages included are described in figure and through the corresponding letter and number designations in the declaration (see
figure below)
Additional technical information:
NEPD-2268-1031-EN OFFECCT Carry On 4 / 8
The following information describe the scenarios in the different modules of the EPD.
The following information describe the scenarios in the different modules of the EPD.
User stage scenario: Estimate done that product needs to be cleaned once per year and possible replacement of fastenings once per life
cycle (15 years). Transport scenario: Transportation to an average customer in Copenhagen is 420km. End of life: Assuming that there will
be legal requirements in the near future for the separation of the constituents we have calculated in step C3 (end of life), the waste process
according to this.
Transport from production place to user (A4)
Capacity
Fuel/Energy
Type utilisation (incl. Type of vehicle Distance km Unit Value (l/t)
consumption
return) %
Truck, 16-32
Truck 38,8 % 420 0,044606 l/tkm 18,73
tonnes, EURO 5
Railway l/tkm
Boat l/tkm
Other Transportation l/tkm
Assembly (A5) End of Life (C1, C3, C4)
. Unit Value . Unit Value
Auxiliary kg Hazardous waste disposed kg
Water consumption m3 Collected as mixed construction waste kg
Electricity consumption kWh Reuse kg
Other energy carriers MJ Recycling kg 1,3400
Material loss kg Energy recovery kg 5,0500
Output materials from waste treatment kg 1,0100 To landfill kg
Dust in the air kg
VOC emissions kg
Transport to waste processing (C2)
Capacity
Fuel/Energy
Type utilisation (incl. Type of vehicle Distance km Unit Value (l/t)
consumption
return) %
Truck, 16-32
Truck 38,8 % 100 0,044606 l/tkm 4,46
tonnes, EURO 5
Railway l/tkm
Boat l/tkm
Other Transportation l/tkm
¨
Benefits and loads beyond the system boundaries (D)
. Unit Value
Substitution of Wood, chipboard (kg) kg/DU 1,00
Substitution of Plastic film, LDPE (kg) kg/DU 0,01
Substitution of Steel, low-alloyed (kg) kg/DU 0,84
Substitution of Polypropylene (kg) kg/DU 0,20
Substitution of Polyethylene HDPE, granulate (kg) kg/DU 0,30
NEPD-2268-1031-EN OFFECCT Carry On 5 / 8
LCA: Results
System boundaries (X=included, MND=module not declared, MNR=module not relevant)
Construction Beyond the
Product stage installation User stage End of life stage . system
stage bondaries
A1 A2 A3 A4 A5 B1 B2 B3 B4 B5 B6 B7 C1 C2 C3 C4 . D
X X X X X MNR MNR MNR MNR MNR MNR MNR X X X MNR . X
Environmental impact
Parameter Unit A1 A2 A3 A4 A5 C1 C2 C3 D
GWP kg CO 2 -eq 2,32E+01 1,94E-01 3,58E-01 4,87E-01 1,68E-02 0 1,16E-01 6,21E+00 -3,40E+00
ODP kg CFC11 -eq 6,75E-07 3,55E-08 3,94E-07 8,98E-08 2,81E-09 0 2,14E-08 2,32E-08 -1,57E-07
POCP kg C 2H 4-eq 7,28E-03 3,16E-05 9,41E-05 7,94E-05 2,72E-06 0 1,89E-05 5,32E-05 -1,73E-03
AP kg SO 2 -eq 1,33E-01 6,42E-04 1,95E-03 1,55E-03 6,23E-05 0 3,70E-04 1,55E-03 -1,49E-02
EP kg PO 3- -eq 1,71E-02 1,13E-04 4,69E-04 2,58E-04 1,37E-05 0 6,14E-05 4,08E-04 -3,15E-03
4
ADPM kg Sb -eq 7,80E-04 6,07E-07 4,66E-06 1,49E-06 5,10E-08 0 3,54E-07 5,75E-07 -3,29E-05
ADPE MJ 2,59E+02 2,91E+00 2,86E+00 7,34E+00 2,43E-01 0 1,75E+00 3,20E+00 -4,05E+01
GWP Global warming potential; ODP Depletion potential of the stratospheric ozone layer; POCP Formation potential of tropospheric photochemical
oxidants; AP Acidification potential of land and water; EP Eutrophication potential; ADPM Abiotic depletion potential for non fossil resources; ADPE
Abiotic depletion potential for fossil resources
Reading example: 9,0 E-03 = 9,0*10-3 = 0,009
*INA Indicator Not Assessed
waR slairetam tropsnarT gnirutcafunaM tropsnarT ylbmessA esU ecnanetniaM riapeR tnemecalpeR tnemhsibrufeR lanoitarepO ygrene esu lanoitarepO esu
retaw
-eD noitcurtsnoc noitilomed tropsnarT etsaW gnissecorp lasopsiD -yrevoceR-esueR -gnilcyceR laitnetop
NEPD-2268-1031-EN OFFECCT Carry On 6 / 8
Resource use
Parameter Unit A1 A2 A3 A4 A5 C1 C2 C3 D
RPEE MJ 1,09E+02 4,28E-02 2,32E+01 1,07E-01 4,73E-03 0 2,55E-02 4,11E+01 -1,51E+01
RPEM MJ 6,87E+01 0,00E+00 0,00E+00 0,00E+00 0,00E+00 0 0,00E+00 0,00E+00 -8,01E+00
TPE MJ 1,78E+02 4,28E-02 2,32E+01 1,07E-01 4,73E-03 0 2,55E-02 4,11E+01 -2,31E+01
NRPE MJ 3,16E+02 2,98E+00 5,24E+01 7,51E+00 2,51E-01 0 1,79E+00 8,64E+01 -4,61E+01
NRPM MJ 5,26E+01 0,00E+00 0,00E+00 0,00E+00 0,00E+00 0 0,00E+00 0,00E+00 -2,03E+01
TRPE MJ 3,68E+02 2,98E+00 5,24E+01 7,51E+00 2,51E-01 0 1,79E+00 8,64E+01 -6,64E+01
SM kg 1,63E+00 0,00E+00 0,00E+00 0,00E+00 0,00E+00 0 0,00E+00 0,00E+00 0,00E+00
RSF MJ 0,00E+00 0,00E+00 2,24E-02 0,00E+00 0,00E+00 0 0,00E+00 0,00E+00 0,00E+00
NRSF MJ 0,00E+00 0,00E+00 0,00E+00 0,00E+00 0,00E+00 0 0,00E+00 0,00E+00 0,00E+00
W m3 2,73E-01 5,59E-04 1,32E-02 1,41E-03 4,87E-05 0 3,35E-04 3,32E-03 -1,47E-02
RPEE Renewable primary energy resources used as energy carrier; RPEM Renewable primary energy resources used as raw materials; TPE Total use
of renewable primary energy resources; NRPE Non renewable primary energy resources used as energy carrier; NRPM Non renewable primary energy
resources used as materials; TRPE Total use of non renewable primary energy resources; SM Use of secondary materials; RSF Use of renewable
secondary fuels; NRSF Use of non renewable secondary fuels; W Use of net fresh water
Reading example: 9,0 E-03 = 9,0*10-3 = 0,009
*INA Indicator Not Assessed
End of life - Waste
Parameter Unit A1 A2 A3 A4 A5 C1 C2 C3 D
HW kg 1,59E-03 1,77E-06 1,91E-05 4,39E-06 1,56E-07 0 1,04E-06 9,47E-06 -1,51E-04
NHW kg 1,17E+01 1,53E-01 3,72E-01 3,95E-01 1,35E-02 0 9,41E-02 4,17E-01 -3,13E+00
RW kg INA* INA* INA* INA* INA* 0 INA* INA* INA*
HW Hazardous waste disposed; NHW Non hazardous waste disposed; RW Radioactive waste disposed
Reading example: 9,0 E-03 = 9,0*10-3 = 0,009
*INA Indicator Not Assessed
End of life - Output flow
Parameter Unit A1 A2 A3 A4 A5 C1 C2 C3 D
CR kg 0,00E+00 0,00E+00 0,00E+00 0,00E+00 0,00E+00 0 0,00E+00 0,00E+00 0,00E+00
MR kg 0,00E+00 0,00E+00 0,00E+00 0,00E+00 1,01E+00 0 0,00E+00 1,29E+00 0,00E+00
MER kg 0,00E+00 0,00E+00 0,00E+00 0,00E+00 5,04E-04 0 0,00E+00 2,52E-02 0,00E+00
EEE MJ INA* INA* INA* INA* INA* 0 INA* INA* INA*
ETE MJ INA* INA* INA* INA* INA* 0 INA* INA* INA*
CR Components for reuse; MR Materials for recycling; MER Materials for energy recovery; EEE Exported electric energy; ETE Exported thermal
energy
Reading example: 9,0 E-03 = 9,0*10-3 = 0,009
*INA Indicator Not Assessed
NEPD-2268-1031-EN OFFECCT Carry On 7 / 8
Additional Norwegian requirements
Greenhouse gas emissions from the use of electricity in the manufacturing phase
National production mix from import, low voltage (production of transmission lines, in addition to direct emissions and losses in grid) of
applied electricity for the manufacturing process (A3).
Electricity mix Data source Amount Unit
El-mix, Sweden (kWh) ecoinvent 3.4 Alloc Rec 42,67 g CO2-ekv/kWh
Dangerous substances
The product contains no substances given by the REACH Candidate list or the Norwegian priority list.
Indoor environment
Additional environmental information
Bibliography
ISO 14025:2010 Environmental labels and declarations - Type III environmental declarations - Principles and procedures.
ISO 14044:2006 Environmental management - Life cycle assessment - Requirements and guidelines.
EN 15804:2012+A1:2013 Environmental product declaration - Core rules for the product category of construction products.
ISO 21930:2017 Sustainability in buildings and civil engineering works - Core rules for environmental product declarations of
construction products.
ecoinvent v3, Allocation, cut-off by classification, Swiss Centre of Life Cycle Inventories.
Iversen et al., (2018) eEPD v3.0 - Background information for EPD generator system. LCA.no report number 04.18
Vold et al., (2019) EPD generator for Norsk Industri, Background information for industry application and LCA data, LCA.no report number
06.19.
NPCR Part A: Construction products and services. Ver. 1.0. April 2017, EPD-Norge.
NPCR 026 PartB forFurniture.Ver.2.0 October2018,EPD-Norge.
Program operator and publisher Phone: +47 23 08 80 00
The Norwegian EPD Foundation
Post Box 5250 Majorstuen, 0303 Oslo e-mail: post@epd-norge.no
0303 Oslo Norway web: www.epd-norge.no
Owner of the declaration Phone:
Flokk Holding AS - OFFECCT Fax:
Grönhultsvägen 3b e-mail: helena.l.aberg@offecct.se
543 51 Tibro, Sweden web: https://www.offecct.com/
Author of the Life Cycle Assessment Phone: +47 916 50 916
LCA.no AS Fax:
Dokka 1C e-mail: post@lca.no
1671 Kråkerøy web: www.lca.no
Developer of EPD generator Phone: +47 916 50 916
LCA.no AS
Dokka 1C e-mail: post@lca.no
1671 Kråkerøy web: www.lca.no
NEPD-2268-1031-EN OFFECCT Carry On 8 / 8
