Environmental product declaration
In accordance with ISO 14025 and EN15804+A2
Ondatherm 1003 PRT Hexacore D=100mm
Owner of the declaration: Program operator:
ArcelorMittal Construction Norge AS The Norwegian EPD Foundation
Product: Declaration number:
Ondatherm 1003 PRT Hexacore D=100mm
NEPD-7364-6743-EN
Declared unit:
1 m2 Registration number:
This declaration is based on Product Category Rules: NEPD-7364-6743-EN
CEN Standard EN 15804:2012+A2:2019 serves as core
Issue date: 26.08.2024
PCR
The Norwegian EPD Foundation
NPCR 013:2021 Part B for Steel and aluminium Valid to: 26.08.2029
construction products
EPD software:
LCAno EPD generator ID: 477384
1 / 12
General information
Product Owner of the declaration:
Ondatherm 1003 PRT Hexacore D=100mm ArcelorMittal Construction Norge AS
Contact person: Stig Tore Sjaastad
Phone: +47 41 723939
e-mail: stig-tore.sjaastad@arcelormittal.com
Program operator: Manufacturer:
The Norwegian EPD Foundation ArcelorMittal Construction Deutschland GmbH
Post Box 5250 Majorstuen, 0303 Oslo, Norway Münchener Straße 2
Phone: +47 977 22 020 06794 Sandersdorf-Brehna, Germany
web: www.epd-norge.no
Declaration number: Place of production:
ArcelorMittal Construction Deutschland GmbH – Werk Brehna
NEPD-7364-6743-EN
Münchener Straße 2
06794 Sandersdorf-Brehna, Germany
This declaration is based on Product Category Rules: Management system:
CEN Standard EN 15804:2012+A2:2019 serves as core PCR ISO 9001, ISO 45001, ISO 50001
NPCR 013:2021 Part B for Steel and aluminium construction products
Statement of liability: Organisation no:
The owner of the declaration shall be liable for the underlying 976289862
information and evidence. EPD Norway shall not be liable with respect
to manufacturer information, life cycle assessment data and
evidences.​
Declared unit: Issue date:
1 m2 Ondatherm 1003 PRT Hexacore D=100mm
26.08.2024
Declared unit with option: Valid to:
A1-A3,A4,A5,C1,C2,C3,C4,D 26.08.2029
Year of study:
2023
Functional unit: Comparability:
EPD of construction products may not be comparable if they not
comply with EN 15804 and seen in a building context.
General information on verification of EPD from EPD tools: Development and verification of EPD:
Independent verification of data, other environmental information The declaration is created using EPD tool lca.tools ver EPD2022.03,
and the declaration according to ISO 14025:2010, § 8.1.3 and § 8.1.4. developed by LCA.no. The EPD tool is integrated in the company's
Verification of each EPD is made according to EPD-Norway’s management system, and has been approved by EPD Norway.
guidelines for verification and approval requiring that tools are i)
integrated into the company's environmental management system, ii) Developer of EPD: Ingo Timmel
the procedures for use of the EPD tool are approved by EPD-Norway,
Reviewer of company-specific input data and EPD:​ Thomas Boehme
and iii) the process is reviewed annually by an independent third
party verifier. See Appendix G of EPD-Norway's General Programme
Instructions for further information on EPD tools
Verification of EPD tool: Approved:
Independent third party verification of the EPD tool, background data
and test-EPD in accordance with EPDNorway's procedures and
guidelines for verification and approval of EPD tools.
Håkon Hauan, CEO EPD-Norge
Third party verifier:
Alexander Borg, Asplan Viak AS
(no signature required)
2 / 12
Product
Product description:
Double skin steel faced sandwich panels with a core made of polyurethane for walls with visible fixing
1 m2 covering surface of Ondatherm 1003 double skin steel faced sandwich panel
The EPD and LCA calculation is based on a standard sandwich panel Ondatherm 1003 with a thickness of 100 mm.
In case a LCA calculation for different sandwich panel thickness is required, please contact the owner of the declaration.
Product specification
- Standard cover width: 1000 mm
- PIR foam: PRT-Hexacore
- Approval: DIBT Z-10.4-913
- Thermal transmittance U = 0.22 W/m²K
- FM certified: 4880 & 4881 & 4882
- Reaction to fire B-s1,d0
- Thicknesses of insulation core available from 40 to 120 mm
- Vertical or horizontal installation
- Visible fixing
Materials kg %
Insulation 3,60 31,66
Metal - Steel 7,77 68,34
Total 11,37 100,00
Packaging kg %
Packaging - Plastic 0,03 42,86
Packaging - Polystyrene 0,04 57,14
Total incl. packaging 11,44 100,00
Technical data:
Ondatherm 1003 sandwich panels fulfill the requirement of the harmonized standard EN 14509
Market:
construction industry, worldwide
Reference service life, product
The expected service life of Ondatherm 1003 is up to 50 years.
Reference service life, building or construction works
The expected service life is set to 50 years for the building in all calculations.
LCA: Calculation rules
Declared unit:
1 m2 Ondatherm 1003 PRT Hexacore D=100mm
Cut-off criteria:
All major raw materials and all the essential energy is included. The production processes for raw materials and energy flows with very small
amounts (less than 1%) are not included. These cut-off criteria do not​ apply for hazardous materials and substances.
Allocation:
The allocation is made in accordance with the provisions of EN 15804. Incoming energy and water and waste production in-house is allocated
equally among all products through mass allocation. Effects of primary production of recycled materials is allocated to the main product in which
the material was used. The recycling process and transportation of the material is allocated to this analysis.
Data quality:
Specific data for the product composition are provided by the manufacturer. The data represent the production of the declared product and were
collected for EPD development in the year of study. Background data is based on EPDs according to EN 15804 and different LCA databases. The
data quality of the raw materials in A1 is presented in the table below.
Materials Source Data quality Year
Insulation INTERNAL LCA STUDY Sphera 2023 2023
Metal - Steel not yet published EPD 0
Packaging - Plastic ecoinvent 3.6 Database 2019
Packaging - Polystyrene ecoinvent 3.6 Database 2019
3 / 12
System boundaries (X=included, MND=module not declared, MNR=module not relevant)
Construction Beyond the system
Product stage Use stage End of life stage
installation stage boundaries
A1 A2 A3 A4 A5 B1 B2 B3 B4 B5 B6 B7 C1 C2 C3 C4 D
X X X X X MND MND MND MND MND MND MND X X X X X
System boundary:
Type of EPD: cradle to gate - with options.
All relevant life cycle stages are covered.
The product stage A1-A3 include the following:
- Production of the raw material
- Transport of the raw material to the fabrication plant
- All production processes in the plant including energy consumption and emissions
- Waste processing until end of waste state or disposal of any waste residues during the production of the sandwich panels
- Production and recycling of packaging
- Manufacturing of the sandwich panel
Module A4:
- delivery to the construction site with a transport distance of 100 km
Module A5:
- disposal of transport packaging at the construction site and energy for installation
The user stage B1-B7 have not been included.
The end of life stage C1-C4:
- include average assumptions, provision for all materials and transports and use of related energy and water
- assumption is made that the PUR/PIR of the sandwich panels will be disposed 100% to landfill
- the steel is fully recyclable in form of scrap by separating the steel sheets from the insulation core
In addition, module D (Beyond the system boundaries) is included.
waR slairetam tropsnarT gnirutcafunaM tropsnarT ylbmessA e​sU ecnanetniaM riapeR tnemecalpeR tnemhsibrufeR lanoitarepO ygrene esu lanoitarepO esu retaw -eD noitcurtsnoc noitilomed tropsnarT etsaW gnissecorp lasopsiD -yrevoceR-esueR laitnetop-gnilcyceR
4 / 12
Additional technical information:
Simplified manufacturing process of Sandwich panels:
In the manufacturing process the raw materials are received and loaded on the production line.
The coloured and organic coated steel sheets undergo a rollforming process and the polyurethan is foamed on the line.
Both components are assembled together during the foaming process and undergo a pressing process afterwards, where pressure and heat with
high temperature are added.
After that the established sandwich panel undergoes a cooling process, where sealing tapes are added and the sandwich panel will be cut to the
desired length ordered by the customer.
Finally, the sandwich panel goes through the stapling and packaging process and will be inspected, before it will be stored for pick-up by the
transport.
5 / 12
LCA: Scenarios and additional technical information
The following information describe the scenarios in the different modules of the EPD.
Capacity utilisation Value
Transport from production place to user (A4) Distance (km) Fuel/Energy Consumption Unit
(incl. return) % (Liter/tonne)
Truck, 16-32 tonnes, EURO 6 (km) 36,7 % 300 0,043 l/tkm 12,90
Assembly (A5) Unit Value
Waste, municipal solid waste, to average
kg 0,04
treatment - A3, A5, inkl. transp. (kg)
Waste, packaging, plastic film (LDPE), to average
kg 0,03
treatment (kg) - A5, inkl. 85 km transp.
De-construction demolition (C1) Unit Value
Demolition of building per kg (kg) kg/DU 11,40
Capacity utilisation Value
Transport to waste processing (C2) Distance (km) Fuel/Energy Consumption Unit
(incl. return) % (Liter/tonne)
Truck, 16-32 tonnes, EURO 6 (km) 36,7 % 100 0,043 l/tkm 4,30
Waste processing (C3) Unit Value
Materials to recycling (kg) kg 6,99
Disposal (C4) Unit Value
Waste, inert waste, to landfill (kg) kg 3,60
Waste, scrap steel, to landfill (kg) kg 0,78
Benefits and loads beyond the system
Unit Value
boundaries (D)
Substitution of primary steel with net scrap (kg) kg 6,61
6 / 12
LCA: Results
The LCA results are presented below for the declared unit defined on page 2 of the EPD document.
Environmental impact
Indicator Unit A1-A3 A4 A5 C1 C2 C3 C4 D
GWP-total kg CO2 -eq 3,48E+01 5,59E-01 2,53E-02 4,56E-02 1,86E-01 0,00E+00 3,29E-02 -7,28E+00
GWP-fossil kg CO2 -eq 3,48E+01 5,59E-01 2,13E-02 4,56E-02 1,86E-01 0,00E+00 3,29E-02 -7,27E+00
GWP-biogenic kg CO2 -eq -6,54E-03 2,31E-04 3,99E-03 8,55E-06 7,71E-05 0,00E+00 3,73E-05 -4,01E-03
GWP-luluc kg CO2 -eq 9,67E-03 1,99E-04 6,75E-07 3,60E-06 6,63E-05 0,00E+00 7,91E-06 -3,26E-03
ODP kg CFC11 -eq 3,83E-05 1,27E-07 4,35E-10 9,85E-09 4,22E-08 0,00E+00 1,28E-08 -2,31E-07
AP mol H+ -eq 7,07E-02 1,61E-03 1,66E-05 4,77E-04 5,35E-04 0,00E+00 2,95E-04 -3,61E-02
EP-FreshWater kg P -eq 2,72E-04 4,46E-06 5,46E-08 1,66E-07 1,49E-06 0,00E+00 3,60E-07 -4,48E-04
EP-Marine kg N -eq 1,73E-02 3,18E-04 1,46E-05 2,11E-04 1,06E-04 0,00E+00 1,10E-04 -7,48E-03
EP-Terrestial mol N -eq 1,83E-01 3,55E-03 6,78E-05 2,28E-03 1,18E-03 0,00E+00 1,21E-03 -7,65E-02
POCP kg NMVOC -eq 6,18E-02 1,36E-03 1,93E-05 6,35E-04 4,54E-04 0,00E+00 3,47E-04 -3,64E-02
ADP-minerals&metals1 kg Sb-eq 3,69E-04 1,54E-05 3,86E-08 7,00E-08 5,14E-06 0,00E+00 2,95E-07 -1,25E-04
ADP-fossil1 MJ 5,37E+02 8,45E+00 3,11E-02 6,28E-01 2,82E+00 0,00E+00 9,20E-01 -6,12E+01
WDP1 m3 8,78E+01 8,17E+00 1,11E-01 1,33E-01 2,72E+00 0,00E+00 5,24E+00 3,77E+02
GWP-total = Global Warming Potential total; GWP-fossil = Global Warming Potential fossil fuels; GWP-biogenic = Global Warming Potential biogenic; GWP-luluc =
Global Warming Potential land use and land use change; ODP = Depletion potential of the stratospheric ozone layer; AP = Acidification potential, Accumulated
Exceedance; EP-freshwater = Eutrophication potential, fraction of nutrients reaching freshwater end compartment: EP-marine = Eutrophication potential, fraction of
nutrients reaching marine end compartment; EP-terrestrial = Eutrophication potential, Accumulated Exceedance; POCP = Formation potential of tropospheric ozone;
ADP-minerals&metals = Abiotic depletion potential for non-fossil resources; ADP-fossil = Abiotic depletion for fossil resources potential; WDP = Water (user)
deprivation potential, deprivation-weighted water consumption
"Reading example: 9,0 E-03 = 9,0*10-3 = 0,009"
*INA Indicator Not Assessed
1. The results of this environmental impact indicator shall be used with care as the uncertainties on these results are high or as there is limited experienced with the
indicator
Remarks to environmental impacts
7 / 12
Additional environmental impact indicators
Indicator Unit A1-A3 A4 A5 C1 C2 C3 C4 D
PM Disease incidence 8,70E-08 3,42E-08 1,91E-10 5,78E-08 1,14E-08 0,00E+00 6,30E-09 -6,04E-07
IRP2 kgBq U235 -eq 1,06E-01 3,69E-02 1,21E-04 2,74E-03 1,23E-02 0,00E+00 4,18E-03 2,61E-02
ETP-fw1 CTUe 1,98E+01 6,26E+00 1,09E-01 3,43E-01 2,09E+00 0,00E+00 4,96E-01 -4,05E+02
HTP-c1 CTUh 2,06E-10 0,00E+00 5,00E-12 1,10E-11 0,00E+00 0,00E+00 2,00E-11 -3,50E-08
HTP-nc1 CTUh 2,08E-08 6,84E-09 1,99E-10 3,19E-10 2,28E-09 0,00E+00 3,51E-10 7,60E-07
SQP1 dimensionless 1,46E+01 5,91E+00 3,43E-02 7,63E-02 1,97E+00 0,00E+00 3,52E+00 -4,58E+00
PM = Particulate Matter emissions; IRP = Ionizing radiation – human health; ETP-fw = Eco toxicity – freshwater; HTP-c = Human toxicity – cancer effects; HTP-nc =
Human toxicity – non cancer effects; SQP = Potential Soil Quality Index (dimensionless)
"Reading example: 9,0 E-03 = 9,0*10-3 = 0,009"
*INA Indicator Not Assessed
1. The results of this environmental impact indicator shall be used with care as the uncertainties on these results are high or as there is limited experienced with the
indicator
2. This impact category deals mainly with the eventual impact of low dose ionizing radiation on human health of the nuclear fuel cycle. It does not consider effects due
to possible nuclear accidents, occupational exposure nor due to radioactive waste disposal in underground facilities. Potential ionizing radiation from the soil, from
radon and from some construction materials is also not measured by this indicator.
8 / 12
Resource use
Indicator Unit A1-A3 A4 A5 C1 C2 C3 C4 D
PERE MJ 2,53E+01 1,21E-01 9,23E-04 3,42E-03 4,03E-02 0,00E+00 3,07E-02 -4,97E+00
PERM MJ 0,00E+00 0,00E+00 0,00E+00 0,00E+00 0,00E+00 0,00E+00 0,00E+00 0,00E+00
PERT MJ 2,53E+01 1,21E-01 9,23E-04 3,42E-03 4,03E-02 0,00E+00 3,07E-02 -4,97E+00
PENRE MJ 5,36E+02 8,45E+00 3,11E-02 6,28E-01 2,82E+00 0,00E+00 9,20E-01 -6,12E+01
PENRM MJ 2,82E+00 0,00E+00 -2,82E+00 0,00E+00 0,00E+00 0,00E+00 0,00E+00 0,00E+00
PENRT MJ 5,38E+02 8,45E+00 -2,79E+00 6,28E-01 2,82E+00 0,00E+00 9,20E-01 -6,12E+01
SM kg 3,99E-01 0,00E+00 0,00E+00 0,00E+00 0,00E+00 0,00E+00 0,00E+00 0,00E+00
RSF MJ 3,34E-01 4,33E-03 2,70E-05 0,00E+00 1,44E-03 0,00E+00 6,38E-04 2,63E-01
NRSF MJ 3,58E-02 1,55E-02 9,87E-05 0,00E+00 5,16E-03 0,00E+00 1,40E-03 7,65E+00
FW m3 1,30E-01 9,03E-04 4,83E-05 3,23E-05 3,01E-04 0,00E+00 1,13E-03 -1,53E-02
PERE = Use of renewable primary energy excluding renewable primary energy resources used as raw materials; PERM = Use of renewable primary energy resources used
as raw materials; PERT = Total use of renewable primary energy resources; PENRE = Use of non renewable primary energy excluding non-renewable primary energy
resources used as raw materials; PENRM = Use of non renewable primary energy resources used as raw materials; PENRT = Total use of non renewable primary energy
resources; SM = Use of secondary materials; RSF = Use of renewable secondary fuels; NRSF = Use of non-renewable secondary fuels; FW = Net use of fresh water
"Reading example: 9,0 E-03 = 9,0*10-3 = 0,009"
*INA Indicator Not Assessed
9 / 12
End of life - Waste
Indicator Unit A1-A3 A4 A5 C1 C2 C3 C4 D
HWD kg 1,86E-03 4,36E-04 7,66E-03 1,85E-05 1,45E-04 0,00E+00 0,00E+00 -3,78E-02
NHWD kg 1,25E+00 4,11E-01 3,76E-02 7,43E-04 1,37E-01 0,00E+00 4,38E+00 -2,97E+00
RWD kg 1,00E-02 5,75E-05 1,08E-07 4,36E-06 1,92E-05 0,00E+00 0,00E+00 2,01E-05
HWD = Hazardous waste disposed; NHWD = Non-hazardous waste disposed; RWD = Radioactive waste disposed
"Reading example: 9,0 E-03 = 9,0*10-3 = 0,009"
*INA Indicator Not Assessed
End of life - Output flow
Indicator Unit A1-A3 A4 A5 C1 C2 C3 C4 D
CRU kg 0,00E+00 0,00E+00 0,00E+00 0,00E+00 0,00E+00 0,00E+00 0,00E+00 0,00E+00
MFR kg 0,00E+00 0,00E+00 1,53E-02 0,00E+00 0,00E+00 6,99E+00 0,00E+00 0,00E+00
MER kg 0,00E+00 0,00E+00 3,47E-02 0,00E+00 0,00E+00 0,00E+00 0,00E+00 0,00E+00
EEE MJ 0,00E+00 0,00E+00 2,06E-02 0,00E+00 0,00E+00 0,00E+00 0,00E+00 0,00E+00
EET MJ 0,00E+00 0,00E+00 3,12E-01 0,00E+00 0,00E+00 0,00E+00 0,00E+00 0,00E+00
CRU = Components for re-use; MFR = Materials for recycling; MER = Materials for energy recovery; EEE = Exported energy electrical; EET = Exported energy thermal
"Reading example: 9,0 E-03 = 9,0*10-3 = 0,009"
*INA Indicator Not Assessed
Biogenic Carbon Content
Indicator Unit At the factory gate
Biogenic carbon content in product kg C 0,00E+00
Biogenic carbon content in accompanying packaging kg C 0,00E+00
Note: 1 kg biogenic carbon is equivalent to 44/12 kg CO2
10 / 12
Additional requirements
Greenhouse gas emissions from the use of electricity in the manufacturing phase
National production mix from import, low voltage (production of transmission lines, in addition to direct emissions and losses in grid) of applied
electricity for the manufacturing process (A3).
Electricity mix Source Amount Unit
Electricity, Germany (kWh) ecoinvent 3.6 585,93 g CO2-eq/kWh
Dangerous substances
The product contains no substances given by the REACH Candidate list.
Indoor environment
Additional Environmental Information
Additional environmental impact indicators required in NPCR Part A for construction products
Indicator Unit A1-A3 A4 A5 C1 C2 C3 C4 D
GWPIOBC kg CO2 -eq 3,49E+01 5,59E-01 2,48E-02 4,56E-02 1,86E-01 0,00E+00 3,29E-02 -1,09E+01
GWP-IOBC: Global warming potential calculated according to the principle of instantaneous oxidation. In order to increase the transparency of biogenic carbon​
contribution to climate impact, the indicator GWP-IOBC is required as it declares climate impacts calculated according to the principle of instantaneous oxidation.​
GWP-IOBC is also referred to as GWP-GHG in context to Swedish public procurement legislation.
11 / 12
Bibliography
ISO 14025:2010 Environmental labels and declarations - Type III environmental declarations - Principles and procedures.
ISO 14044:2006 Environmental management - Life cycle assessment - Requirements and guidelines.
EN 15804:2012+A2:2019 Environmental product declaration - Core rules for the product category of construction products.
ISO 21930:2017 Sustainability in buildings and civil engineering works - Core rules for environmental product declarations of construction
products.
ecoinvent v3, Allocation, cut-off by classification, Swiss Centre of Life Cycle Inventories.
Iversen et al., (2021) eEPD v2021.09 Background information for EPD generator tool system verification, LCA.no Report number: 07.21
Graafland and Iversen, (2022) EPD generator for EPD generator for NPCR 013 Part B for Steel and Aluminum, Background information for EPD
generator application and LCA data, LCA.no report number: 08.22
NPCR Part A: Construction products and services. Ver. 2.0. April 2021, EPD-Norge.
NPCR 013 Part B for Steel and Aluminium Construction Products , Ver. 4.0, 06.10.2021, EPD Norway.
Program operator and publisher Phone: +47 977 22 020
The Norwegian EPD Foundation e-mail: post@epd-norge.no
Post Box 5250 Majorstuen, 0303 Oslo, Norway web: www.epd-norge.no
Owner of the declaration: Phone: +47 41 723939
stig-
ArcelorMittal Construction Norge AS e-mail:
tore.sjaastad@arcelormittal.com
Sørumgata 11A, 2000 Lillestrøm web:
Author of the Life Cycle Assessment Phone: +47 916 50 916
LCA.no AS e-mail: post@lca.no
Dokka 6A, 1671 web: www.lca.no
Developer of EPD generator Phone: +47 916 50 916
LCA.no AS e-mail: post@lca.no
Dokka 6B,1671 Kråkerøy web: www.lca.no
ECO Platform web: www.eco-platform.org
ECO Portal web: ECO Portal
12 / 12
