ENVIRONMENTAL PRODUCT DECLARATION
as per ISO 14025 and EN 15804+A2
Owner of the Declaration Sonae Arauco, S.A.
Publisher Institut Bauen und Umwelt e.V. (IBU)
Programme holder Institut Bauen und Umwelt e.V. (IBU)
Declaration number EPD-SON-20220209-ICC2-EN
Issue date 06.09.2022
Valid to 05.09.2027
Oriented Strand Board
Sonae Arauco, S.A.
www.ibu-epd.com | https://epd-online.com
1. General Information
Sonae Arauco, S.A. Oriented Strand Board
Programme holder Owner of the declaration
IBU – Institut Bauen und Umwelt e.V. Sonae Arauco, S.A.
Hegelplatz 1 Centro Empresarial Euronova, C/Ronda de Poniente, 6 ­ B
10117 Berlin 28760 Tres Cantos (Madrid)
Germany Spain
Declaration number Declared product / declared unit
EPD­SON­20220209­ICC2­EN AGEPAN® OSB ECOBOARD and OSB ECOBOARD (Oriented Strand
Board), per m3
This declaration is based on the product category rules: Scope:
Wood­based panels, 01.08.2021 This document refers to sanded and unsanded OSB manufactured in the
(PCR checked and approved by the SVR) following plant of the Sonae Arauco group:
Sonae Arauco Deutschland GmbH
Issue date Strohmweg 1
D­38489 Nettgau
06.09.2022
Germany
The production volume of this plant covers 100 % of the total production of
Valid to
OSB by Sonae Arauco group.
05.09.2027 The owner of the declaration shall be liable for the underlying information
and evidence; the IBU shall not be liable with respect to manufacturer
information, life cycle assessment data and evidences.
The EPD was created according to the specifications of EN 15804+A2. In
the following, the standard will be simplified as EN 15804.
Verification
The standard EN 15804 serves as the core PCR
Independent verification of the declaration and data according to ISO
14025:2011
Dipl.­Ing. Hans Peters internally X externally
(Chairman of Institut Bauen und Umwelt e.V.)
Florian Pronold Dr. Stefan Diederichs,
(Managing Director Institut Bauen und Umwelt e.V.) (Independent verifier)
1 Environmental Product Declaration ­ Sonae Arauco, S.A. ­ Oriented Strand Board
2. Product
Performance data of the product in accordance with the
2.1 Product description/Product definition declaration of performance with respect to its essential
AGEPAN® OSB ECOBOARD and OSB ECOBOARD (Oriented characteristics according to EN 300: 1996, Oriented Strand
Strand Board) are wood materials comprising large longitudinal Boards (OSB) – Definitions, classification and specifications.
wood shavings ("strands") which are glued with formaldehyde­
free glue, using a synthetic resin binding agent (pMDI). The For more details on technical information, please see the
strands are aligned in a process­controlled manner (oriented) AGEPAN® OSB ECOBOARD and OSB ECOBOARD
and compressed in a continuous process (ContiRoll Declaration of Performance (DoP) at:
technology) in three layers, ranging in thickness from 6 to 40 www.sonaearauco.com/dop
mm. The upper and lower layers are longitudinal while the
middle layer runs transversally to the panel direction. 2.4 Delivery status
The gross densities of OSB are dependent on the quality
Both AGEPAN® OSB ECOBOARD and OSB ECOBOARD (OSB/1 – OSB/4) and thickness and are between 590 and 640
focus on construction, as part of Sonae Arauco solutions for kg/m³. Boards of 6 mm to 40 mm thickness are manufactured in
this application. For the placing on the market of the product in various standard formats or to special customer specifications.
the European Union/European Free Trade Association
(EU/EFTA) (with the exception of Switzerland) Regulation (EU) Thickness 6 ­ 40 mm
No. 305/2011 (CPR) applies. The product needs a declaration Width 590 ­ 1250 mm
of performance taking into consideration EN 300: 1996, Length 1840 ­ 6250 mm
Oriented Strand Boards (OSB) – Definitions, classification and
specifications and the CE­marking. For updated information on available dimensions, please refer
For the application and use, national provisions existing in each to www.agepan.de/produkt
country can apply.
2.5 Base materials/Ancillary materials
2.2 Application AGEPAN® OSB ECOBOARD and OSB ECOBOARD with
AGEPAN® OSB ECOBOARD and OSB ECOBOARD have a thicknesses of 6 to 40 mm with an average density of 601 kg/m³
comprise (details provided as mass % per 1 m³ of product):
high load capacity and are dimensionally stable. They can be
used for both constructive and decorative purposes. • Wood chips, primarily softwood, > 90%
A prerequisite for constructive application is represented by the • Water (moisture), approx. 3% to 6%
performance characteristics of EN 13986 and the CE mark. • pMDI adhesive (polymer 4.4' diphenyl methane
Areas of application include: supporting and bracing wall and diisocyanate), approx. 3% to 4.5%
ceiling paneling, floor installations and installation panels, shop • Paraffin wax emulsion, 0.5% to 2.5%
and trade fair stand construction as well as packaging and Logs from indigenous, largely regional forestry plantations are
furniture elements. used for manufacturing AGEPAN® OSB ECOBOARD and OSB
Various OSB qualities manufactured by Sonae Arauco are ECOBOARD. The wood is procured from forests within a radius
numbered 2 to 4 according to EN 300. of approx. 130 km of the plant location.
When wood imports are required, the average wood
The following classifications apply for various applications: procurement distances (to the plant) increase to around 200km.
· OSB/2: Panels for load­bearing use in dry conditions Short transport routes make a particular contribution towards
· OSB/3: Panels for load­bearing use in humid conditions minimising CO2 emissions and the logistical effort involved in
· OSB/4: Panels for heavy duty load­bearing purposes for use the provision of raw materials.
in humid conditions The entire OSB product range is PEFC™ certified. FSC®
certified products can be made available on request.
2.3 Technical Data
This product contains substances listed in the ECHA candidate
Values list (date: 08.06.2021) exceeding 0.1 percentage by mass:
cover OSB/2, OSB/3 and OSB/4:
Name Value Unit · no
Gross density according to EN 300 > 600 kg/m3
This product contains other carcinogenic, mutagenic, reprotoxic
Bending strength (longitudinal) according to
14 ­ 25 N/mm2 (CMR) substances in categories 1A or 1B which are not on the
EN 300
ECHA candidate list, exceeding 0.1 percentage by mass:
Bending strength (transverse) according to
7 ­ 13 N/mm2
EN 300 · no
4930 ­
E­module (longitudinal) according to EN 300 N/mm2
6780 Biocide products were added to this construction product or it
1980 ­ has been treated with biocide products (this then concerns a
E­module (transverse) according to EN 300 N/mm2
2680 treated product as defined by the (EU) Ordinance on Biocide
Products No. 528/2012:
Material dampness at delivery ­ %
Thermal conductivity according to EN 13986 0.13 W/(mK)
· no
Water vapour diffusion resistance factor
150 ­
according to EN 13986 (only for OSB/3 and ­ 2.6 Manufacture
250
OSB/4) The manufacturing of OSB comprises the following steps:
Sound absorption coefficient ­ %
Formaldehyde emissions acc. to EN 717­1 < 62,0 μg/m3 1. Debarking the logs
2. Chipping the wood in the knife ring flaker
2 Environmental Product Declaration ­ Sonae Arauco, S.A. ­ Oriented Strand Board
3. Drying
4. Sifting in top and middle layer fractions A process diagram is presented below.
5. Interim storage in proportioning hoppers
6. Weight determination of strands with scale The production site is certified according to the following
7. Separate glueing of the top and middle layer strands standards:
8. Scattering the OSB mat (alignment of the strands)
• ISO 9001
9. Compressing the OSB mat under high pressure in a
• ISO 45001
continuous hot press
• ISO 50001
10. Cooling the raw boards in star coolers
Additionally, all range includes CE marked products, and
11. Stacking
PEFCTM and FSC® certified products can be made available
12. Optional: Sanding the top and underside
on request.
13. Optional: Distribution into fixed formats or tongue and
groove panels
appropriately by structural measures.
2.7 Environment and health during manufacturing
Health protection: Due to the manufacturing conditions, no The production site is ISO 14001 certified.
special health protection measures over and beyond the
regulatory guidelines are required. The reference occupational 2.8 Product processing/Installation
exposure limit values are complied with. AGEPAN® OSB ECOBOARD and OSB ECOBOARD can be
sawn, drilled and milled using standard (electric) power tools.
Emissions into air: Waste air generated during production is Carbide­tipped tools should be given preference, especially on
cleaned in accordance with regulatory specifications. Emissions circular saws. Respiratory protection should be worn when
are below the limit values specified by the operation license of using hand­held equipment without suction devices.
the site, specified according to German law.
2.9 Packaging
Emissions into water/soil: No normal process contamination Particleboard, OSB and corrugated cardboard are used for
of water or soil exists. The production site does not have any covering while PET or steel tape packing bands are used for
production­related waste water. packing.
If re­use or recycling is impractical, the packaging should not be
Noise: Sound protection analyses have established that all landfilled, but rather directed towards energy recovery.
values communicated inside and outside the production
2.10 Condition of use
facilities are below the standards applicable in Germany. Noise­
intensive plant areas such as chipping are encapsulated
3 Environmental Product Declaration ­ Sonae Arauco, S.A. ­ Oriented Strand Board
The materials used in AGEPAN® OSB ECOBOARD and OSB excluding flooring
ECOBOARD comply with the percentages indicated in 2.5., applications, and for thicknesses ≥ 9 mm without air gap behind
whereby a polyurethane resin is used as a binding agent for the the OSB material or with closed or open air gap not more than
boards with a formaldehyde­free glueing system. 22 mm behind)
VOC emissions: AGEPAN® OSB ECOBOARD and OSB
ECOBOARD are labelled as class A according to the French Water
regulation on the labelling of emissions of volatile pollutants No ingredients are washed out which could be hazardous to
from construction and decoration products (with reference to water. OSB boards are not resistant to permanent exposure to
the wall scenario, as a worst case). water; damaged areas can however be replaced locally.
Additionally, parts of the range for AGEPAN® OSB ECOBOARD
Mechanical destruction
and OSB ECOBOARD have been certified with the IBU
OSB board breakage features display relatively brittle
environmental quality label.
performance, whereby sharp edges can arise on the broken
AGEPAN® OSB ECOBOARD and OSB ECOBOARD at an
panel edges.
average density of 601 kg/m3 store 987 kg CO2­eq/m3 over
their service life. 2.14 Re-use phase
OSB untreated boards can be re­used for the same or similar
2.11 Environment and health during use
application as long as they are collected separately.
Environmental protection: According to current information,
water, air and soil are not exposed to any danger when
Recycling: AGEPAN® OSB ECOBOARD and OSB
AGEPAN® OSB ECOBOARD and OSB ECOBOARD boards
ECOBOARD boards from construction and any other
are used as designated.
application can be collected separately and utilized in the
manufacture of particleboard. This is based on the condition
Health protection: According to current information, no
that the wooden boards are not fully glued or treated with
damage to or impairment of health can be anticipated when
hazardous chemicals
AGEPAN® OSB ECOBOARD and OSB ECOBOARD boards
are used as designated.
Energy recovery: due to the high heating value of approx. 16.0
2.12 Reference service life MJ/kg at an assumed end­of­life moisture content of 20 %,
Due to the wide range of applications AGEPAN® OSB AGEPAN® OSB ECOBOARD and OSB ECOBOARD boards
can be used for energy recovery and the generation of heat
ECOBOARD and OSB ECOBOARD,
and electricity (e.g. in CHP plants), following the cascading
no reference service life is declared.
principle for wood.
2.13 Extraordinary effects
2.15 Disposal
Fire
OSB leftovers and residual materials incurred as a result of
Fire retardant classification of AGEPAN® OSB ECOBOARD
demolition measures on the building site should be primarily
and OSB ECOBOARD boards is done according to EN 13986.
directed towards material recycling. If this is not possible, they
Fire retardant classes defined in accordance with EN 13501-1.
must be directed toward energy recovery instead of landfilling.
Fire protection
Name Value Waste code according to the European List of Waste: 17 02 01
Building material class D
2.16 Further information
Smoke gas development S2
Further information such as technical datasheets etc. can be
Burning droplets d0 downloaded under:
www.sonaearauco.com
3. LCA: Calculation rules
manufacturing of the products, including raw material extraction
3.1 Declared Unit and processing, energy generation, the production of ancillary
The declared unit for the LCA is 1 m3 of AGEPAN® OSB products and packaging materials, transport, as well as all
ECOBOARD and OSB ECOBOARD. waste treatment processes. Eventual benefits of recycling or
The indicator values represent an average product of a density energy recovery are neglected.
of 601 kg/m3, which represents the (slightly rounded) weighted The resource aspects of wood were inventoried via material
production mix of the reference year 2020. inherent properties such as resource extraction of CO from the
2
Information on the declared unit atmosphere and the lower heating value as the use of
renewable energy.
Name Value Unit
Material inherent properties are subject to co­product allocation
Declared unit 1 m3
as ruled in EN 15804.
Mass reference 601 kg/m3
Module A4 covers the transport of the product from the
production site to the construction site by a lorry over a default
3.2 System boundary distance of 460 km.
Type of the EPD: cradle­to­gate with modules C1 to C4 and Module A5 covers the transport of the packaging material from
module D (A1­A3, C and D) the construction site and its disposal. Default end­of­waste
states for the packaging materials from the packed products at
Modules A1 – A3 of the production stage cover the the construction site are defined in analogy for wastes
occurring in modules A1­A3. Eventual further inputs for the
4 Environmental Product Declaration ­ Sonae Arauco, S.A. ­ Oriented Strand Board
installation of the products are not considered due to the broad Beyond that, no material or energy flows were neglected that
applicability of the assessed products. would have been known by the persons responsible for the
The substituted primary material from the net amount of project and that could have been expected to contribute
recycled material and from recovered energy exported from the significantly to the environmental indicators declared. It can
product system in Module A5 is declared in Module D. thus be assumed that the total contribution of the neglected
processes is not higher than 5 % of the declared impact
Module C1 manual deconstruction is assumed. The declared categories.
values are thus 0.
3.5 Background data
Module C2 includes the transport of the de­constructed product Datasets from ecoinvent 3.7.1 were used as background data
to a recycling centre by over 50 km. exclusively. Therefore, the latest update of the background data
took place in 2020.
Module C3 covers the preparation of the post­consumer board
3.6 Data quality
to become a secondary fuel; the end­of­waste status for
recycled wood­based boards is defined as the point where they The requirements on the data quality and the background data
have been sorted and chipped, ready to be used as secondary correspond to the provisions in EN 15804 and the IBU PCR
fuels. part A (IBU 2020) respectively:
In line with EN 16485, the export of the biogenic carbon stored • Data are as current as possible. Datasets used for
in the board, expressed in CO ­equivalent is also reported in calculations were updated within the last 10 years for
2
module C3. generic data and within the last 5 years for producer­
specific data;
Module C4 is not relevant for the assumed end­of­life scenario.
The declared values are thus 0. • Datasets are based on 1 year averaged data as a
Module D compiles all the benefits and burdens associated with general rule;
the secondary fuels, secondary materials and exported energy
leaving the production system in the modules A5 and C3. • The time period over which inputs to and outputs from
the system are accounted for is 100 years from the year
Therefore, module D covers the avoided burdens from recycling for which the data set is deemed representative;
and from energy recovered from the waste treatment in module
A5 as well as the transport of the obsolete boards to a biomass • The technological coverage reflects the physical reality
combustion plant, the combustion process itself and the loads of the declared products;
and benefits of the substitution of fossil fuels and/or electricity.
Substitution effects in module D are always calculated for the • The background datasets comply with the quality
net amount of secondary material or secondary fuel of the guidelines of ecoinvent 3.7.1; deviations from the
product system in line with EN 16485. methodological prescriptions of EN 15804 and the IBU
PCR part A (IBU 2020) respectively are possible but
3.3 Estimates and assumptions acceptable according to IBU PCR part A (IBU 2020).
For the quantification of the net flows of recycled wood (input of
post­consumer wood used as a fuel minus post­consumer 3.7 Period under review
wood exiting the product system into module D for energy The company data gathered for this EPD represents the year
recovery), it was assumed that all inputs of post­consumer 2020.
wood are used as a fuel.
3.8 Geographic Representativeness
Beyond that, no relevant estimates or assumptions had to be
made beyond the information provided in this EPD. Land or region, in which the declared product system is
manufactured, used or handled at the end of the product´s
3.4 Cut-off criteria lifespan: Germany
The applicable criteria for the exclusion of inputs and outputs
are defined in EN 15804, clause 6.3.6, and in the IBU PCR part
3.9 Allocation
A (IBU 2020), respectively.
Specific data for the production line for the production of OSB
All data were taken into account that resulted from the data
was available for all relevant inputs. Airborne emissions were
collection procedure in the plants, e.g., related to fuels, raw
attributed based on the relative energy consumption of the
material input, use of ancillary materials, waste flows,
different products produced in the plant, except for
emissions into air, water use, waste water, transport means and
formaldehyde, which was allocated to the products using UF
transport distances, etc.
glues.
Expenses for the general management, research &
development, administration and marketing – if known – were
The inventories for the wood inputs were taken from ecoinvent
not taken into account.
3.7.1, based on Werner et al. 2015. In these datasets, resource
The production of eventual packaging of ancillary material or
corrections are made for incorporated biogenic carbon and
other inputs used during production (and some of the reported
renewable energy; these flows thus reflect the real physical
wastes) was generally neglected; in most cases reusable bins
flows.
or containers are used. In addition, the amounts of reported
(unspecific) wastes are so small that their production can be
No post­consumer secondary wood is used as an input to
considered not relevant for the life cycle assessment.
produce the OSB; for the end­of­life scenario, the end­of­waste
Beyond that some ancillary materials were cut off due to very
status was defined after the sorting and chipping of the wood­
small amounts and as inputs not directly related to production
based board in line with EN 16485 (see also clause 3.2). Loads
processes but to the maintenance of infrastructure, e.g.,
and benefits of energy recovery are thus reported in module D.
acetylene and oxygen for soldering, etc.
Waste packaging in module A5 was considered not to reach the
With this approach also mass and energy flows below 1 percent
end­of­waste state as a fuel. Its incineration is reported in A5,
of total mass and energy flows caused by the declared
the benefits of energy recovery in module D. The benefits of the
products were included in the assessment.
5 Environmental Product Declaration ­ Sonae Arauco, S.A. ­ Oriented Strand Board
recycling of a minor amount of cardboard packaging are possible if all the data sets to be compared were created
disregarded. according to EN 15804 and the building context, respectively
No co­product allocation was made in the modelling of the life the product­specific characteristics of performance, are taken
cycle assessment underlying this EPD. into account. ecoinvent 3.7.1 has been used as the background
database
3.10 Comparability
Basically, a comparison or an evaluation of EPD data is only
4. LCA: Scenarios and additional technical information
waste input; 92 % of the recovered energy is heat, 8 % is
Characteristic product properties of biogenic carbon electricity (according to specifications of MWI plants in
ecoinvent 3.7.1).
Information on describing the biogenic carbon content at
factory gate Deconstruction (C1)
manual deconstruction is assumed. The declared values are
Name ValueUnit
thus 0.
kg
Biogenic carbon content in product 284
C
Transport to waste treatment (C2)
Biogenic carbon content in accompanying kg This module includes the transport of the de­constructed
4,22
packaging C product to a recycling center by a lorry (15 % emissions class
EURO 5; 85% emissions class EURO 6) by over 50 km.
The following technical information is a basis for the declared
Waste treatment (C3)
modules or can be used for developing specific scenarios in the
601 kg of OSB are chipped and exported from the product life
context of a building assessment if modules are not declared
cycle into module D, assuming a moisture content of 20 % and
(MND).
a lower heating value of 15.7 MJ/kg. The biogenic carbon
stored in the product and the content of primary energy are
Transport to the construction site (A4)
exported from the product system as material inherent
The product is transported from the production site to the
properties.
construction site by a lorry (15 % emissions class EURO 5;
85% emissions class EURO 6) over a default distance of 460
Disposal (C4)
km.
This module is not relevant for the assumed end­of­life
scenario. The declared values are thus 0.
Installation into the building (A5)
Eventual further inputs for the installation of the products are
Reuse, recycling, recovery potential (D)
not considered due to the broad applicability of the assessed
According to default assumptions in other IBU EPDs, post­
products.
consumer wood is used as a secondary fuel for energy
An average transport distance of 30 km was assumed for
recovery in a biomass combustion plant with an overall energy
packaging waste from the construction site to the recycling
efficiency of 93 % related to the lower heating value of the fuel
plant or to the municipal waste incineration plant. The municipal
input; 91 % of the recovered energy is heat, 9 % is electricity.
waste incineration plant is assumed to have an overall energy
efficiency of 53 % related to the lower heating value of the
6 Environmental Product Declaration ­ Sonae Arauco, S.A. ­ Oriented Strand Board
5. LCA: Results
DESCRIPTION OF THE SYSTEM BOUNDARY (X = INCLUDED IN LCA; ND = MODULE OR INDICATOR NOT DECLARED; MNR =
MODULE NOT RELEVANT)
Benefits and
Construction loads beyond
Product stage Use stage End of life stage
process stage the system
boundaries
la ire ta m w a Ry lp p u s tro p s n a rT g n iru tc a fu n a M e h t m o rf tro p s n a rTe tis e h t o t e ta g y lb m e s s A e s U e c n a n e tn ia M ria p e R tn e m e c a lp e R tn e m h s ib ru fe R y g re n e la n o ita re p Oe s u re ta w la n o ita re p Oe s u n o itc u rts n o c ­e Dn o itilo m e d tro p s n a rT g n is s e c o rp e ts a W la s o p s iD ­e s u e R­y re v o c e R­g n ilc y c e Rla itn e to p
A1 A2 A3 A4 A5 B1 B2 B3 B4 B5 B6 B7 C1 C2 C3 C4 D
X X X X X MND MND MNR MNR MNR MND MND X X X X X
RESULTS OF THE LCA - ENVIRONMENTAL IMPACT according to EN 15804+A2: AGEPAN® OSB ECOBOARD and OSB
ECOBOARD, per m³
Parameter Unit A1-A3 A4 A5 C1 C2 C3 C4 D
GWP­total kg CO 2 eq ­6.58E+02 4.58E+01 1.66E+01 0 6.4E+00 9.91E+02 0 ­5.33E+02
GWP­fossil kg CO 2 eq 3.41E+02 4.58E+01 1.46E+00 0 6.4E+00 5.11E+00 0 ­5.32E+02
GWP­biogenic kg CO 2 eq ­1E+03 0 1.52E+01 0 0 9.86E+02 0 0
GWP­luluc kg CO 2 eq 2.04E+00 1.57E­02 4.6E­04 0 2.67E­03 1.03E­02 0 ­2.1E­01
ODP kg CFC11 eq 5.67E­05 1.04E­05 2.51E­07 0 1.41E­06 2.6E­07 0 ­7.82E­05
AP mol H+ eq 1.57E+00 1.36E­01 6.35E­03 0 1.87E­02 2.72E­02 0 ­5.99E­01
EP­freshwater kg P eq 2.73E­02 3.42E­04 1.66E­05 0 5.49E­05 5.29E­04 0 ­1.04E­02
EP­marine kg N eq 4.87E­01 3.05E­02 2.48E­03 0 4.04E­03 3.73E­03 0 ­4.17E­02
EP­terrestrial mol N eq 4.26E+00 3.38E­01 2.78E­02 0 4.49E­02 4.23E­02 0 ­4.63E­01
kg NMVOC
POCP 2.13E+00 1.22E­01 8.27E­03 0 1.62E­02 1.18E­02 0 ­2.51E­01
eq
ADPE kg Sb eq 2.48E­03 1.68E­04 4.44E­06 0 3.04E­05 1.27E­05 0 ­2.44E­04
ADPF MJ 6.41E+03 6.94E+02 9.33E+00 0 9.58E+01 1.05E+02 0 ­1.03E+04
m3 world eq
WDP 1.06E+02 2E+00 2.91E­01 0 3.01E­01 1.09E+00 0 ­1.81E+01
deprived
GWP = Global warming potential; ODP = Depletion potential of the stratospheric ozone layer; AP = Acidification potential of land and water; EP =
Eutrophication potential; POCP = Formation potential of tropospheric ozone photochemical oxidants; ADPE = Abiotic depletion potential for non­fossil
resources; ADPF = Abiotic depletion potential for fossil resources; WDP = Water (user) deprivation potential)
RESULTS OF THE LCA - INDICATORS TO DESCRIBE RESOURCE USE according to EN 15804+A2: AGEPAN® OSB
ECOBOARD and OSB ECOBOARD, per m³
Parameter Unit A1-A3 A4 A5 C1 C2 C3 C4 D
PERE MJ 1.41E+04 9.3E+00 1.9E+02 0 1.52E+00 1.62E+01 0 ­3.3E+02
PERM MJ 1E+04 0 ­1.9E+02 0 0 ­9.85E+03 0 0
PERT MJ 2.41E+04 9.3E+00 4.57E­01 0 1.52E+00 ­9.83E+03 0 ­3.3E+02
PENRE MJ 5.34E+03 6.95E+02 1.86E+01 0 9.59E+01 1.06E+02 0 ­1.03E+04
PENRM MJ 1.1E+03 0 ­9.24E+00 0 0 ­1.09E+03 0 0
PENRT MJ 6.43E+03 6.95E+02 9.35E+00 0 9.59E+01 ­9.81E+02 0 ­1.03E+04
SM kg 0 0 0 0 0 0 0 3.85E­01
RSF MJ 0 0 0 0 0 0 0 9.85E+03
NRSF MJ 0 0 0 0 0 0 0 1.09E+03
FW m3 3.05E+00 7.26E­02 1.08E­02 0 1.08E­02 6.02E­02 0 ­8.9E­01
PERE = Use of renewable primary energy excluding renewable primary energy resources used as raw materials; PERM = Use of renewable primary
energy resources used as raw materials; PERT = Total use of renewable primary energy resources; PENRE = Use of non­renewable primary energy
excluding non­renewable primary energy resources used as raw materials; PENRM = Use of non­renewable primary energy resources used as raw
materials; PENRT = Total use of non­renewable primary energy resources; SM = Use of secondary material; RSF = Use of renewable secondary fuels;
NRSF = Use of non­renewable secondary fuels; FW = Use of net fresh water
RESULTS OF THE LCA – WASTE CATEGORIES AND OUTPUT FLOWS according to EN 15804+A2:
AGEPAN® OSB ECOBOARD and OSB ECOBOARD, per m³
Parameter Unit A1-A3 A4 A5 C1 C2 C3 C4 D
HWD kg 8.63E­03 1.81E­03 9.48E­06 0 2.56E­04 4.2E­05 0 ­1.1E­02
NHWD kg 5.82E+01 3.39E+01 2E­01 0 3.82E+00 6.55E­01 0 1.72E+00
RWD kg 3.6E­02 1.02E­02 1.08E­04 0 1.39E­03 1.34E­03 0 ­3.41E­02
CRU kg 0 0 0 0 0 0 0 0
MFR kg 0 0 3.85E­01 0 0 0 0 0
MER kg 0 0 0 0 0 6.01E+02 0 0
EEE MJ 0 0 6.62E+00 0 0 0 0 0
7 Environmental Product Declaration ­ Sonae Arauco, S.A. ­ Oriented Strand Board
EET MJ 0 0 7.6E+01 0 0 0 0 0
HWD = Hazardous waste disposed; NHWD = Non­hazardous waste disposed; RWD = Radioactive waste disposed; CRU = Components for re­use;
MFR = Materials for recycling; MER = Materials for energy recovery; EEE = Exported electrical energy; EET = Exported thermal energy
RESULTS OF THE LCA – additional impact categories according to EN 15804+A2-optional:
AGEPAN® OSB ECOBOARD and OSB ECOBOARD, per m³
Parameter Unit A1-A3 A4 A5 C1 C2 C3 C4 D
Disease
PM ND ND ND ND ND ND ND ND
incidence
IR kBq U235 eq 1.55E+01 3.05E+00 3.92E­02 0 4.22E­01 9.1E­01 0 ­1.98E+01
ETP­fw CTUe 1.22E+04 5.33E+02 7.19E+01 0 7.65E+01 5.86E+01 0 ­1E+03
HTP­c CTUh 2.49E­06 1.89E­08 2.76E­09 0 3.04E­09 3.5E­09 0 1.41E­07
HTP­nc CTUh 2.3E­05 5.24E­07 2.42E­08 0 7.09E­08 4.66E­08 0 ­3.83E­07
SQP SQP 1.28E+05 4.84E+02 2.19E+00 0 5.68E+01 1.54E+01 0 ­3.34E+02
PM = Potential incidence of disease due to PM emissions; IR = Potential Human exposure efficiency relative to U235; ETP­fw = Potential comparative
Toxic Unit for ecosystems; HTP­c = Potential comparative Toxic Unit for humans (cancerogenic); HTP­nc = Potential comparative Toxic Unit for humans
(not cancerogenic); SQP = Potential soil quality index
ND: emissions of particulate matter (PM) are not declared due to inconsistencies in the reported data.
Disclaimer 1 – for the indicator 'potential Human exposure efficiency relative to U235'.This impact category deals mainly with the
eventual impact of low­dose ionizing radiation on human health of the nuclear fuel cycle. It does not consider effects due to possible
nuclear accidents, occupational exposure or radioactive waste disposal in underground facilities. Potential ionizing radiation from the
soil, radon and from some construction materials is also not measured by this indicator.
Disclaimer 2 – for the indicators: 'abiotic depletion potential for fossil resources', 'abiotic depletion potential for non­fossil resources',
'water (user) deprivation potential', 'deprivation­weighted water consumption', 'potential comparative toxic unit for ecosystems',
'potential comparative toxic unit for humans ­ cancer effects', 'potential comparative toxic unit for humans – non­cancer effects',
'potential soil quality index'.The results of this environmental impact indicator shall be used with care as the uncertainties on these
results are high or as there is limited experience with the indicator.
6. LCA: Interpretation
Indicators of the impact assessment the overall indicator results of the impact assessment (impact
from modules A1 ­ C4 = 100 %).
Figure 1 illustrates the contribution of each life cycle stage to
Figure 1 illustrates that the impacts over the life cycle of the
Figure 1: Environmental impacts of AGEPAN® OSB product are predominantly caused during the production of the
ECOBOARD and OSB ECOBOARD along its life cycle OSB; the impacts from other parts of the life cycle are not
(impacts from production modules A1-C4 = 100 %) significant.
8 Environmental Product Declaration ­ Sonae Arauco, S.A. ­ Oriented Strand Board
accumulation of nutrients in soils and watersheds, which can
For the GWP, the ODP and the ADP fossil, the benefits from the cause increased growth of algae and shifts in species
energy recovery of AGEPAN® OSB ECOBOARD and OSB composition.
ECOBOARD are higher than the impacts during the life cycle, The EP is caused by a variety of processes, mainly in
notably the impacts from production; for other impact combustion processes or disposal processes, e.g., of mining
categories, the benefits of energy recovery lie between 10 % to residues from lignite extraction related to the generation of
35 %, depending on the impact category under consideration. electricity.
The EP is caused mainly by airborne emissions of nitrogen
The global warming potential (GWP) is an indicator for the oxides as well as phosphate emissions into the groundwater.
contribution to climate change and is quan­tified based on the
emissions of gases that absorb radiative forcing. The photochemical oxidation potential (POCP) assesses the
The production phase of AGEPAN® OSB ECOBOARD and contribution of airborne emissions that contribute to summer
OSB ECOBOARD is largely caused by the upstream processes ozone creation.
of the production of PMDI (around 35 %); the use of natural gas
during production and the generation of electricity cause About 30 % of the POCP are associated with the production of
another 17 % of the GWP each; in sum, 20 % of the GWP are PMDI resins and with on­site emissions during the production of
related to the forestry processes and by the transport for raw the AGEPAN® OSB ECOBOARD and OSB ECOBOARD;
material acquisition. another 30% are caused by harvesting operations of stem
Figure 2 illustrates that the biogenic carbon stored in the wood. These contributions are caused by emissions of SO 2,
product, expressed as CO 2­equivalent, is higher than the CO 2 CO and CH 4.
emissions from fossil sources, leading to a negative GWP for
the production mod­ule A1­A3. The potential substitution effect The abiotic resource depletion potential of fossil resources
in module D more than offsets the GHG emissions during the (ADP fossil) assesses the use of scarce fossil resources such
production phase (module A1­A3). as natural gas or crude oil.
The GWP is dominated by CO 2 emissions and removals. The ADP (fossil resources) is caused mainly by the production
of PMDI (40 %), the on­site consumption of natural gas (15 %)
and by the generation of electricity.
The abiotic resource depletion potential for mineral resource
(ADP elements) assesses the use of scarce mineral resources
such as ores and other mineral raw materials.
The ADP (elements) is caused almost completely by
infrastructure processes, such as the buildings required for the
production of chemicals; the main resources contributing to the
ADP (elements) are copper, zinc and gold.
Selected indicators from the life cycle inventory
The main use of renewable primary energy is the heating value
of the wood in AGEPAN® OSB ECOBOARD and OSB
ECOBOARDB; this amount of non­used renewable energy is
Figure 2: Carbon footprint of AGEPAN® OSB ECOBOARD
exported in module C3 and used energetically as a renewable
and OSB ECOBOARD
secondary fuel in module D. The renewable primary energy
used as energy is mainly woody biomass.
The ozone layer depletion potential (ODP) is quantified based
The major share of the non­renewable primary energy is used
on the emissions of gases that can de­stroy stratospheric
energetically, mainly as natural gas in the upstream processes
ozone.
for the production of PMDI. A minor share is used as a material,
The ODP is caused mainly by emissions of Halon 1211, which
i.e., as com­po­nents of the gluing systems; this non­renewable
are associated with the production and transport of natural gas.
primary energy used as a material is not used within the life
Around 15 % of the ODP are associated with the use of natural
cycle of AGEPAN® OSB ECOBOARD and OSB ECOBOARDS;
gas on­site for the production of AGEPAN® OSB ECOBOARD
it is exported in module C3 and used energetically as a non­
and OSB ECOBOARDB, the rest of the ODP is caused by the
renewable secondary fuel in module D.
use of natural gas in upstream processes in line with the
consumption patterns of natural gas in the process chain,
The indicator values for wastes refer to the amount of waste
notably for the production of PMDI.
that is landfilled after an eventual pre­treatment of the wastes.
The acidification potential (AP) is created with the
The main part of the wastes associated with the production of
transformation of airborne emissions into acids, which among
OSB is non­hazardous waste, mainly resulting from the
other can reduce soil fertility.
disposal of infrastructure associated with, e.g., production halls
Roughly, 15% of the AP are caused by the on­site combustion
or roads.
processes for the production of heat and electricity; the other
Hazardous wastes are generated throughout the production
85 % are associated with upstream combustion processes,
chain, e.g., related to disposal of ashes, production wastes
notably for heat production in the production of the PMDI (50
from chemical industry or from the production of primary
%), for the generation of electricity (10 %), and related to the
aluminium for infrastruc­ture processes.
transport of raw materials.
The generation of radioactive waste is associated with the
The AP is caused in comparable shares by emissions of
production of nuclear power.
ammonia, nitrogen oxides and sulphur dioxide.
The net consumption of fresh water is caused mainly by cooling
The various eutrophication potentials (EP) quantify the
processes throughout the production chain as well as partly for
9 Environmental Product Declaration ­ Sonae Arauco, S.A. ­ Oriented Strand Board
the generation of electricity. values that result from the inventorying of waste streams into
thermal waste treatment, energy recovery and recycling.
The further indicators on environmental aspects are singular
7. Requisite evidence
7.1 Formaldehyde Measuring agency: MPA Eberswalde, Materialprüfanstalt
Brandenburg GmbH, Germany.
AGEPAN® OSB ECOBOARD and OSB ECOBOARD meet the
requirements of the German Chemicals Prohibition Regulation Test report reference: 31/18/3277/15A issued 2019,
(ChemVerbotsV)
AGEPAN® OSB ECOBOARD and OSB ECOBOARD TVOC
ZE05 Certificates by MPA Eberswalde, Materialprüfanstalt emissions were determined according to ISO16000-1, with the
Brandenburg GmbH, Germany. wall panel loading scenario and a load facto of 1.00 m2/m3
OSB2 ZE05/20/3949/01 issued 2020
OSB3 ZE05/20/3950/01 issued 2020 Measuring agency: Fraunhofer Institute for Wood Research,
OSB4 ZE05/20/3951/01 issued 2020 Wilhelm­Klauditz­Institut (WKI)
Test reports by measuring agency: MPA Eberswalde, Test report reference: MAIC­2019­3255 issued 2019
Materialprüfanstalt Brandenburg GmbH, Germany.
AgBB overview of results (3 days [µg/m³])
Name Value Unit
Test reports:
OSB2 test report 31/21/ 3949/ 01 QT issued 2021 TVOC (C6 ­ C16) 430 μg/m3
OSB3 test report 31/21/3950/01 QT issued 2021 Sum SVOC (C16 ­ C22) < 5 * μg/m3
OSB4 test report 31/21/3951/01 QT issued 2021
R (dimensionless) 954 ­
VOC without NIK ­ μg/m3
The determination of the formaldehyde content according to
DIN EN 717-1 (chamber method) for AGEPAN® OSB Carcinogenic Substances ­ μg/m3
ECOBOARD and OSB ECOBOARD are below 0.062 mg/m3,
AgBB overview of results (28 days [µg/m³])
complying with the E1 requirements of EN 13986. 7.2. MDI
This test is not required by the applicable product standard. Name Value Unit
TVOC (C6 ­ C16) 430 μg/m3
Measuring agency: Wessling – engineering consultants, Sum SVOC (C16 ­ C22) < 5 * μg/m3
Altenberge, Germany
R (dimensionless) 0.954 ­
Test report, date: IAL­10­0078 OSB (d = 15 mm), dated 12 VOC without NIK ­ μg/m3
January 2010 Carcinogenic Substances ­ μg/m3
* below detection limits
Result: Examination of wood­based materials in a test chamber
(MDI). The test was carried out in accordance with the test
7.5 PCP/Lindane
guidelines stipulated by the RAL-UZ-76 (wood­based
materials). Emissions of monomer MDI and other isocyanates
Measuring agency: MPA Eberswalde, Materialprüfanstalt
could not be determined in the test chamber. The limit of
Brandenburg GmbH, Germany
detection was 0.1 µg/m3. 7.3 Checking for the pre-treatment
of the substances used
Test report reference:
No post­consumer wood is used in the production of AGEPAN®
OSB ECOBOARD and OSB ECOBOARD. . 7.4 TVOC
OSB2 test report 31/21/3949/01 PL issued 2021
emissions
OSB3 test report 31/21/3950/02 PL issued 2021
AGEPAN® OSB ECOBOARD and OSB ECOBOARD boards
OSB4 test report 31/21/3951/02 PL issued 2021
are labelled as class A according to the French regulation on
the labelling of emissions of volatile pollutants (with reference to
Result: The analysis values are under the limit of detection of
the wall scenario, as a worst case).
0.10 mg/kg (process: CEN/TR 14823, EN 322).
Measuring agency: MPA Eberswalde, Materialprüfanstalt
7.6 Heavy metals migration
Brandenburg GmbH, Germany.
Test report according to EN 71-3
Test report reference: OSB3 test report 31/18/3277/14A
Measuring agency: ÜV Rheinland LGA Products GmbH
issued 2019
Test report reference: 0001091206/10 AZ 415482a issued
AGEPAN® OSB ECOBOARD and OSB ECOBOARD meet the
2021
requirements of the MVV TB, Appendix 8 ABG applied in
Germany.
Result: Compliance with all limit values established by EN 71-3
was confirmed, among which Arsenic, Aluminium, Barium,
Attestation reference: OSB_VOC_Gutachten_G­160­18­0003
Cadmium, Chromium, Copper Lead, Mercury and Zinc.
by Deutsches Institut für Bautechnik (DIBt)
8. References
10 Environmental Product Declaration ­ Sonae Arauco, S.A. ­ Oriented Strand Board
Product category rules of IBU EN 13501­1:2019­05, Fire classification of construction
products and building elements – Classification using test data
IBU (2021) from reaction to fire tests.
IBU (2021): General Instructions for the EPD Programme of the
Institut Bauen & Umwelt e.V. (General Instructions for the IBU EN 13986
EPD Programme). Version 2.0, Institut Bauen & Umwelt, Berlin. EN 13986:2015, Wood­based panels for use in construction –
Characteristics, evaluation of conformity and marking.
IBU (2021)
IBU (2021): PCR Part A: Calculation rules for the life cycle EN 300
assessment and requirements for the project report according EN 300: 2006, Oriented Strand Boards (OSB) – Definitions,
to EN 15804+A2:2019. Version 2.1., Institut Bauen & Umwelt, classification and specifications.
Berlin.
EN 16485
IBU (2019) EN 16485:14­07, Round and sawn timber – Environmental
Institut Bauen und Umwelt e.V, Berlin (pub.): Product Category Product Declarations – Product category rules for wood and
Rules for Construction Products from the range of wood­based products for use in construction.
Environmental Product Declarations for Institut Bauen und
Umwelt (IBU), Part B: Requirements on the EPD of wood based EN ISO 50001
panels, 2019­01. EN ISO 50001:2018­12, Energy management systems –
Requirements with guidance for use.
Standards and legal documents
Regulation No. 305/2011
EN 15804 Regulation No. 305/2011 (Construction Products Regulation, or
EN 15804+A2:2019, Sustainability of construction works ­ CPR) of the European Parliament and of the European Council
Environmental product declarations ­ Core rules for the product is a regulation of 9 March 2011 that lays down harmonised
category construction products. conditions for the marketing of construction products and
replaces Construction Products Directive (89/106/EEC).
ISO 14025
ISO 14025:2006­07, Environmental labels and declarations ­ ECHA candidate list
Type III Environmental declarations ­ Principles and Candidate List of substances of very high concern for
procedures. Authorisation, published in accordance with Article 59(10) of the
REACH Regulation. European Chemicals Agency, Brussels.
ISO 14044
EN ISO 14044:2006­07, Environmental management ­ Life Ordinance on Biocide Products No. 528/2012
cycle assessment ­ Requirements and guidance (ISO REGULATION (EU) No 528/2012 OF THE EUROPEAN
14044:2006); German and English versions EN ISO PARLIAMENT AND OF THE COUNCIL of 22 May 2012
14044:2006. concerning the making available on the market and use of
biocidal products.
ISO 9001
ISO 9001:2015, Quality management systems – Requirements. European List of Waste
Commission Decision of 3 May 2000 replacing Decision
ISO 14001 94/3/EC establishing a list of wastes pursuant to Article 1(a) of
ISO 14001:2015, Environmental management systems – Council Directive 75/442/EEC on waste and Council Decision
Requirements with guidance for use. 94/904/EC establishing a list of hazardous waste pursuant to
Article 1(4) of Council Directive 91/689/EEC on hazardous
OHSAS 18001 waste (notified under document number C(2000) 1147).
OHSAS 18001:2007, Occupational Health and Safety
Management Systems – Requirements. Additional references
ISO 45001 ecoinvent 3.7.1
ISO 45001:2018:03, Occupational health and safety Life cycle inventory data, December 2020. Ecoinvent Center,
management systems ­ Requirements with guidance for use. Zurich.
ISO 16000 Werner et al. 2015
ISO 16000­11:2006, Indoor air – Part 11: Determination of the Werner F., Bauer C., Büsser S., Doka G., Kaufmann E., Kono
emission of volatile organic compounds from building products J., Luginbühl, U., Mina M., Frischknecht R., Thees O, Wallbaum
and furnishing – Sampling, storage of samples and preparation H., Zimmermann W., Hischier R. (2014): Aktualisierung der
of test specimens. Modelle und Datensätze zu Holz und Holzprodukten in der
Datenbank ecoinvent. Commissioner: Bundesamt für Umwelt,
EN 717-1 Aktionsplan Holz, Bern. Final report 18. February 2015.
EN 717­1:2005­01, Wood­based panels – Determination of The literature referred to in the Environmental Product
formaldehyde release – Formaldehyde emission by the Declaration must be listed in full.Standards already fully quoted
chamber method. in the EPD do not need to be listed here again.
The current version of PCR Part A and PCR Part B of the PCR
EN 13501 document on which they are based must be referenced.
11 Environmental Product Declaration ­ Sonae Arauco, S.A. ­ Oriented Strand Board
Publisher
Institut Bauen und Umwelt e.V. +49 (0)30 3087748­ 0
Hegelplatz 1 info@ibu­epd.com
10117 Berlin www.ibu­epd.com
Germany
Programme holder
Institut Bauen und Umwelt e.V. +49 (0)30 3087748­ 0
Hegelplatz 1 info@ibu­epd.com
10117 Berlin www.ibu­epd.com
Germany
Author of the Life Cycle Assessment
Dr. Frank Werner ­ Umwelt & Entwicklung + 41 (0)44 241 39 06
Idaplatz 3 frank@frankwerner.ch
8003 Zürich http://www.frankwerner.ch/
Switzerland
Owner of the Declaration
Sonae Arauco, S.A. (+34) 918 070 701
Centro Empresarial Euronova, C/Ronda de products@sonaearauco.com
Poniente, 6 ­ B www.sonaearauco.com
28760 Tres Cantos (Madrid)
Spain
12 Environmental Product Declaration ­ Sonae Arauco, S.A. ­ Oriented Strand Board
