Environmental product declaration
in accordance with ISO 14025 and EN 15804+A2
Outlet +S 2 pole with switch + earth 1.5M
Owner of the declaration: Program operator:
SG Armaturen AS The Norwegian EPD Foundation
Product: Declaration number:
Outlet +S 2 pole with switch + earth 1.5M
NEPD-8201-7867-EN
Declared unit:
1 pcs Registration number:
This declaration is based on Product Category Rules: NEPD-8201-7867-EN
CEN Standard EN 15804:2012+A2:2019
Issue date: 22.11.2024
PCR EPD Italy 007 - Electronic and electrical products and
The Norwegian EPD Foundation systems - Other electronics Valid to: 22.11.2029
EPD software:
LCAno EPD generator ID: 609210
1 / 12
General information
Product Owner of the declaration:
Outlet +S 2 pole with switch + earth 1.5M SG Armaturen AS
Contact person: Audun Skare
Phone: +47 90021243
e-mail: audun.skare@sg-as.no
Program operator: Manufacturer:
The Norwegian EPD Foundation SG Armaturen AS
Post Box 5250 Majorstuen, 0303 Oslo, Norway Skytterheia 25
Phone: +47 977 22 020 4790 Lillesand, Norway
web: www.epd-norge.no
Declaration number: Place of production:
SG Armaturen production site FT (China)
NEPD-8201-7867-EN
, China
This declaration is based on Product Category Rules: Management system:
CEN Standard EN 15804:2012+A2:2019
PCR EPD Italy 007 - Electronic and electrical products and systems -
Other electronics
Statement of liability: Organisation no:
The owner of the declaration shall be liable for the underlying 958560931
information and evidence. EPD Norway shall not be liable with respect
to manufacturer information, life cycle assessment data and
evidences.​
Declared unit: Issue date:
1 pcs Outlet +S 2 pole with switch + earth 1.5M 22.11.2024
Declared unit with option: Valid to:
A1,A2,A3,A4,A5,C1,C2,C3,C4,D 22.11.2029
Year of study:
2023
Functional unit: Comparability:
1 pc Outlet +S 2 pole with Switch w/Earth 1,5M manufactured and EPD of construction products may not be comparable if they not
installed, including waste treatment at end-of-life. comply with EN 15804 and seen in a building context.
General information on verification of EPD from EPD tools: Development and verification of EPD:
Independent verification of data, other environmental information The declaration is created using EPD tool lca.tools ver EPD2022.03,
and the declaration according to ISO 14025:2010, § 8.1.3 and § 8.1.4. developed by LCA.no. The EPD tool is integrated in the company's
Verification of each EPD is made according to EPD-Norway’s management system, and has been approved by EPD Norway.
guidelines for verification and approval requiring that tools are i) NEPDT63
integrated into the company's environmental management system, ii)
the procedures for use of the EPD tool are approved by EPD-Norway, Developer of EPD: Benedikte Ruud Andersen
and iii) the process is reviewed annually by an independent third
Reviewer of company-specific input data and EPD:​ Audun Skare
party verifier. See Appendix G of EPD-Norway's General Programme
Instructions for further information on EPD tools
Verification of EPD tool: Approved:
Independent third party verification of the EPD tool, background data
and test-EPD in accordance with EPDNorway's procedures and
guidelines for verification and approval of EPD tools. Approval
number: NEPDT78.
Third party verifier:
Elisabet Amat, GREENIZE projects
(no signature required)
2 / 12
Product
Product description:
Outlet with switch +S design for fixed installations. 100% compatible with both new and old boxes and frames. Lightning fast assembly via SG's
unique push clamp terminals fastening in the box via wedges, which do not fall off unless desired, and Torx 10 screws for the box. Front plastic is
included and is made of color-resistant and antibacterial plastic that does not fade in color and helps keep touch surfaces clean and bacteria-free.
Voltage: 250V. Current: 10A. Material: Anti-bacterial UV Resistant PC. Colour: White RAL 9016. Indoor. Length (mm): 72. Width (mm): 45. Height
(mm): 35. EAN: 7021985181013.
The EPD also covers the following products:
EAN: 7021985180016 - DOUBLE OUTLET +S 2-POLE WITH SWITCHES 1.5M WHITE
EAN: 7021985180115 - DOUBLE OUTLET +S 2-POLE WITH SWITCHES 1.5M ANTRACIT
EAN: 7021985181112 - OUTLET +S 2 POLE WITH SWITCH + DK EARTH 1.5M ANTRACIT
EAN: 7021985182010 - OUTLET +S 2 POLE WITH SWITCH 1.5M WHITE
EAN: 7021985182119 - OUTLET +S 2 POLE WITH SWITCH 1.5M ANTRACIT
Product specification
Materials kg %
Metal - Copper 0,01 20,63
Metal - Steel low alloy 0,00 3,23
Plastic - Nylon (PA) 0,00 1,07
Rubber, synthetic 0,00 0,18
Metal - Brass 0,00 6,57
Metal - Stainless steel 0,00 4,10
Plastic - Polycarbonate (PC) 0,04 64,22
Total 0,06 100,00
Packaging kg %
Packaging - Cardboard 0,00 14,55
Packaging - Paper 0,00 81,61
Packaging - Recycled paper 0,00 3,84
Total incl. packaging 0,06 100,00
Technical data:
Declaration data:
Standards:
EN 60884-1:2013 (applies to plugs and fixed or portable socket-outlets for AC only, with or without earthing contact for household and similar
purposes, either indoors or outdoors)
Link to product data on our website:
https://www.sg-as.com/da/produkter/stikkontakt-med-afbryder-s/7021985181013/pdf/specifikation_7021985181013.pdf
Market:
Nordic + Northwestern Europe.
Reference service life, product
20 years. Estimated based on the characteristics of the product and the intended application.
Reference service life, building or construction works
60 years. Standard service life for buildings to the PCR Part A of EPD Norway.
LCA: Calculation rules
Declared unit:
1 pcs Outlet +S 2 pole with switch + earth 1.5M
Cut-off criteria:
All major raw materials and all the essential energy is included. The production processes for raw materials and energy flows with very small
amounts (less than 1%) are not included. These cut-off criteria do not​ apply for hazardous materials and substances.
Allocation:
3 / 12
The allocation is made in accordance with the provisions of EN 15804. Incoming energy and water and waste production in-house is allocated
equally among all products through mass allocation. Effects of primary production of recycled materials is allocated to the main product in which
the material was used. The recycling process and transportation of the material is allocated to this analysis.
Data quality:
Specific data for the product composition are provided by the manufacturer. The data represent the production of the declared product and were
collected for EPD development in the year of study. Background data is based on EPDs according to EN 15804 and different LCA databases. The
data quality of the raw materials in A1 is presented in the table below.
Materials Source Data quality Year
Metal - Brass Modified ecoinvent 3.6 Database 2019
Metal - Copper ecoinvent 3.6 Database 2019
Metal - Stainless steel ecoinvent 3.6 Database 2019
Metal - Steel low alloy ecoinvent 3.6 Database 2019
Packaging - Cardboard Modified ecoinvent 3.6 Database 2019
Packaging - Paper ecoinvent 3.6 Database 2019
Packaging - Recycled paper Modified ecoinvent 3.6 Database 2019
Plastic - Nylon (PA) ecoinvent 3.6 Database 2019
Plastic - Polycarbonate (PC) ecoinvent 3.6 Database 2019
Rubber, synthetic ecoinvent 3.6 Database 2019
4 / 12
System boundaries (X=included, MND=module not declared, MNR=module not relevant)
Construction Beyond the system
Product stage Use stage End of life stage
installation stage boundaries
A1 A2 A3 A4 A5 B1 B2 B3 B4 B5 B6 B7 C1 C2 C3 C4 D
X X X X X MND MND MND MND MND MND MND X X X X X
System boundary:
Additional technical information:
Link to Mounting instruction on our website:
https://www.sg-as.com/storage/data/703230_Stik%20med%20afbryderS%20DK/20/703230_Stikkontakt_User%20Manual.pdf
waR slairetam tropsnarT gnirutcafunaM tropsnarT ylbmessA e​sU ecnanetniaM riapeR tnemecalpeR tnemhsibrufeR lanoitarepO ygrene esu lanoitarepO esu retaw -eD noitcurtsnoc noitilomed tropsnarT etsaW gnissecorp lasopsiD -yrevoceR-esueR laitnetop-gnilcyceR
5 / 12
LCA: Scenarios and additional technical information
The following information describe the scenarios in the different modules of the EPD.
Module A4 = Transportation by truck (160 km) from the production site in Shunde, China to the harbor in Shenzhen, China. After this the goods
are transported by ship (19330 km) from Shenzhen, China to Hamburg, Germany. Then with a truck (650 km) from Hamburg, Germany to the
warehouse in Lillesand, Norway + 800 km for Nordic / Northwestern Europe Market.
Modules A5 = Installation is performed in the Nordic / Northwestern Europe Market and done by manual labor. The use of portable electrical
devices such as drills usually have low energy requirements falling under the cut-off criterion of 1% and are therefore neglected (especially for
small retail switches, outlets etc.). No product scraps are generated during installation, but the end-of-life treatment of packaging is systematically
accounted for in this module.
Module B1-B7 have been excluded since the product(s) covered by this EPD do not contain electronic components or due to the absence of clear
and standardized guidelines to calculate impacts during the use phase.
Module C1 = De-installation is done by manual labor. The use of portable electrical devices such as drills usually have low energy requirements
falling under the cut-off criterion of 1% and are therefore neglected (especially for small retail switches).
Module C2 = Transportation from building site to the waste treatment facility with an average distance of 300km.
Modules C3 and C4 = Waste treatment of the product follows the default values provided in EN 50693, Product Category Rules for life cycle
assessments of electronic and electrical products and systems, table G.4. This table specified how different types of raw materials used in A1 will
likely be treated during the end-of-life of the product. Waste treatments in C3 include material recycling and incineration with energy recovery and
fly ash extraction. Disposal in C4 consist of landfilling of different waste fractions and of ashes.
Module D = The recyclability of metals, plastics, and electronic components allows the producers a credit for the net scrap that is produced at the
end of a product’s life. The benefits from recycling of net scrap are described in formula from EN 15804:2012+A2:2019. Substitution of heat and
electricity generated by the incineration with energy recovery of plastic insulation and other parts is also calculated in module D.
Capacity utilisation Value
Transport from production place to user (A4) Distance (km) Fuel/Energy Consumption Unit
(incl. return) % (Liter/tonne)
Ship, Freight, Transoceanic (km) 65,0 % 19330 0,003 l/tkm 57,99
Truck, 16-32 tonnes, EURO 6 (km) - Europe 36,7 % 1450 0,043 l/tkm 62,35
Truck, 16-32 tonnes, EURO 6 (km) - Rest of World 38,8 % 160 0,044 l/tkm 7,04
Assembly (A5) Unit Value
Waste, packaging, kraft paper, unbleached, to
average treatment (kg) - Global - A5, incl. 85 km kg 0,00
transp.
Waste, packaging, corrugated board box, with
recycled content, to average treatment (kg) - A5 kg 0,00
including transport
Waste, packaging, paper printed, 100% recycled
content, to average treatment (kg) - Global - A5, kg 0,00
incl. 85 km transp
Capacity utilisation Value
Transport to waste processing (C2) Distance (km) Fuel/Energy Consumption Unit
(incl. return) % (Liter/tonne)
Truck, 16-32 tonnes, EURO 6 (km) - Europe 36,7 % 300 0,043 l/tkm 12,90
Waste processing (C3) Unit Value
Steel to recycling (kg) kg 0,00
Copper to recycling (kg) kg 0,01
Waste treatment of plastic mixture, incineration
kg 0,02
with energy recovery and fly ash extraction (kg)
Brass to recycling (kg) kg 0,00
Disposal (C4) Unit Value
Landfilling of steel (kg) kg 0,00
Landfilling of copper (kg) kg 0,00
Landfilling of ashes from incineration of Plastic
kg 0,00
mixture, process per kg ashes and residues (kg)
Landfilling of plastic mixture (kg) kg 0,02
Landfilling of brass (kg) kg 0,00
Benefits and loads beyond the system
Unit Value
boundaries (D)
Substitution of primary steel with net scrap (kg) kg 0,00
Substitution of primary copper with net scrap (kg) kg 0,00
Substitution of electricity (MJ) MJ 0,03
Substitution of thermal energy, district heating
MJ 0,43
(MJ)
Substitution of primary Brass with net scrap (kg) kg 0,00
6 / 12
LCA: Results
The LCA results are presented below for the declared unit defined on page 2 of the EPD document.
Environmental impact
Indicator Unit A1 A2 A3 A4 A5 C1 C2 C3 C4 D
GWP-total
kg CO2 -
4,78E-01 2,81E-03 1,39E-01 2,70E-02 7,28E-03 0 2,97E-03 4,36E-02 2,21E-03 -1,29E-02
eq
GWP-fossil
kg CO2 -
4,81E-01 2,81E-03 1,39E-01 2,70E-02 6,74E-05 0 2,96E-03 4,36E-02 2,21E-03 -1,28E-02
eq
GWP-biogenic
kg CO2 -
-3,43E-03 1,09E-06 4,02E-05 9,60E-06 7,21E-03 0 1,23E-06 9,48E-07 1,89E-07 -4,96E-05
eq
GWP-luluc
kg CO2 -
2,29E-04 1,03E-06 1,69E-05 1,33E-05 2,23E-08 0 1,06E-06 1,77E-07 8,02E-08 -9,74E-05
eq
kg
ODP CFC11 - 1,13E-08 6,07E-10 1,20E-09 5,94E-09 1,40E-11 0 6,72E-10 9,70E-11 8,20E-11 -1,81E-04
eq
mol H+
AP 8,79E-03 8,39E-06 6,89E-04 4,04E-04 3,19E-07 0 8,52E-06 9,56E-06 2,21E-06 -1,26E-03
-eq
EP-FreshWater kg P -eq 7,75E-05 2,63E-08 2,86E-06 1,76E-07 5,54E-10 0 2,37E-08 8,41E-09 3,72E-09 -8,98E-06
EP-Marine kg N -eq 5,28E-04 1,65E-06 1,41E-04 9,71E-05 1,06E-07 0 1,69E-06 4,57E-06 2,98E-06 -6,14E-05
mol N -
EP-Terrestial 6,70E-03 1,85E-05 1,56E-03 1,08E-03 1,14E-06 0 1,89E-05 4,69E-05 8,83E-06 -9,02E-04
eq
kg
POCP NMVOC 2,13E-03 6,92E-06 4,04E-04 2,93E-04 3,28E-07 0 7,22E-06 1,13E-05 2,96E-06 -2,47E-04
-eq
ADP- kg Sb-
1,24E-04 7,52E-08 3,55E-07 5,22E-07 1,64E-09 0 8,19E-08 4,77E-09 2,16E-09 -2,43E-05
minerals&metals1 eq
ADP-fossil1 MJ 5,67E+00 4,14E-02 1,16E+00 3,82E-01 9,43E-04 0 4,48E-02 6,00E-03 6,55E-03 -1,35E-01
WDP1 m3 4,66E-01 1,35E-02 1,12E-01 2,46E-01 1,19E-03 0 4,34E-02 4,33E-02 9,55E-02 -8,51E-02
GWP-total = Global Warming Potential total; GWP-fossil = Global Warming Potential fossil fuels; GWP-biogenic = Global Warming Potential biogenic; GWP-luluc =
Global Warming Potential land use and land use change; ODP = Depletion potential of the stratospheric ozone layer; AP = Acidification potential, Accumulated
Exceedance; EP-freshwater = Eutrophication potential, fraction of nutrients reaching freshwater end compartment: EP-marine = Eutrophication potential, fraction of
nutrients reaching marine end compartment; EP-terrestrial = Eutrophication potential, Accumulated Exceedance; POCP = Formation potential of tropospheric ozone;
ADP-minerals&metals = Abiotic depletion potential for non-fossil resources; ADP-fossil = Abiotic depletion for fossil resources potential; WDP = Water (user)
deprivation potential, deprivation-weighted water consumption
"Reading example: 9,0 E-03 = 9,0*10-3 = 0,009"
*INA Indicator Not Assessed
1. The results of this environmental impact indicator shall be used with care as the uncertainties on these results are high or as there is limited experienced with the
indicator
Remarks to environmental impacts
The product is compliant with the European RoHS Directive 2011/65/EU on Restriction of the use of certain Hazardous Substances in Electrical and
Electronic equipment and with the European REACH regulation (EC) no 1907/2006 on Registration, Evaluation, Authorization and Restriction of
Chemicals.
7 / 12
Additional environmental impact indicators
Indicator Unit A1 A2 A3 A4 A5 C1 C2 C3 C4 D
PM Disease incidence 4,18E-08 1,81E-10 9,27E-09 9,83E-10 5,00E-12 0 1,82E-10 4,20E-11 4,00E-11 -3,88E-09
IRP2 kgBq U235 -eq 5,80E-03 1,72E-04 8,32E-04 1,65E-03 4,03E-06 0 1,96E-04 1,51E-05 3,60E-05 -4,36E-04
ETP-fw1 CTUe 6,87E+01 3,36E-02 3,48E+00 2,62E-01 1,26E-03 0 3,32E-02 9,22E-02 4,31E+00 -1,17E+01
HTP-c1 CTUh 1,62E-09 0,00E+00 3,40E-11 0,00E+00 0,00E+00 0 0,00E+00 2,00E-12 0,00E+00 -1,75E-10
HTP-nc1 CTUh 1,19E-07 3,10E-11 1,48E-09 1,94E-10 1,00E-12 0 3,60E-11 1,16E-10 6,00E-12 -1,38E-08
SQP1 dimensionless 2,02E+00 2,84E-02 2,48E-01 1,87E-01 6,32E-04 0 3,14E-02 1,10E-03 2,01E-02 -3,82E-01
PM = Particulate Matter emissions; IRP = Ionizing radiation – human health; ETP-fw = Eco toxicity – freshwater; HTP-c = Human toxicity – cancer effects; HTP-nc =
Human toxicity – non cancer effects; SQP = Potential Soil Quality Index (dimensionless)
"Reading example: 9,0 E-03 = 9,0*10-3 = 0,009"
*INA Indicator Not Assessed
1. The results of this environmental impact indicator shall be used with care as the uncertainties on these results are high or as there is limited experienced with the
indicator
2. This impact category deals mainly with the eventual impact of low dose ionizing radiation on human health of the nuclear fuel cycle. It does not consider effects due
to possible nuclear accidents, occupational exposure nor due to radioactive waste disposal in underground facilities. Potential ionizing radiation from the soil, from
radon and from some construction materials is also not measured by this indicator.
8 / 12
Resource use
Indicator Unit A1 A2 A3 A4 A5 C1 C2 C3 C4 D
PERE MJ 4,03E-01 4,69E-04 1,17E-01 4,33E-03 1,55E-05 0 6,42E-04 3,34E-04 5,19E-04 -2,50E-01
PERM MJ 5,38E-02 0,00E+00 0,00E+00 0,00E+00 -5,38E-02 0 0,00E+00 0,00E+00 0,00E+00 0,00E+00
PERT MJ 4,57E-01 4,69E-04 1,17E-01 4,33E-03 -5,38E-02 0 6,42E-04 3,34E-04 5,19E-04 -2,50E-01
PENRE MJ 4,74E+00 4,14E-02 1,16E+00 3,82E-01 9,43E-04 0 4,48E-02 6,00E-03 6,55E-03 -1,35E-01
PENRM MJ 9,35E-01 0,00E+00 0,00E+00 0,00E+00 0,00E+00 0 0,00E+00 -9,35E-01 0,00E+00 0,00E+00
PENRT MJ 5,67E+00 4,14E-02 1,16E+00 3,82E-01 9,43E-04 0 4,48E-02 -9,29E-01 6,55E-03 -1,35E-01
SM kg 9,03E-03 0,00E+00 0,00E+00 0,00E+00 0,00E+00 0 0,00E+00 0,00E+00 0,00E+00 1,38E-03
RSF MJ 1,59E-03 9,17E-06 5,65E-05 1,40E-04 5,15E-07 0 2,30E-05 7,17E-06 1,08E-05 1,01E-04
NRSF MJ 2,25E-03 7,79E-05 6,81E-04 7,64E-04 2,12E-06 0 8,21E-05 0,00E+00 8,91E-06 -1,11E-02
FW m3 4,09E-03 4,63E-06 1,09E-03 3,32E-05 4,45E-07 0 4,79E-06 5,07E-05 8,31E-06 -4,78E-04
PERE = Use of renewable primary energy excluding renewable primary energy resources used as raw materials; PERM = Use of renewable primary energy resources used
as raw materials; PERT = Total use of renewable primary energy resources; PENRE = Use of non renewable primary energy excluding non-renewable primary energy
resources used as raw materials; PENRM = Use of non renewable primary energy resources used as raw materials; PENRT = Total use of non renewable primary energy
resources; SM = Use of secondary materials; RSF = Use of renewable secondary fuels; NRSF = Use of non-renewable secondary fuels; FW = Net use of fresh water
"Reading example: 9,0 E-03 = 9,0*10-3 = 0,009"
*INA Indicator Not Assessed
9 / 12
End of life - Waste
Indicator Unit A1 A2 A3 A4 A5 C1 C2 C3 C4 D
HWD kg 1,38E-03 3,75E-06 2,00E-04 1,94E-05 0,00E+00 0 2,31E-06 0,00E+00 2,78E-04 -1,04E-04
NHWD kg 4,90E-02 1,99E-03 1,40E-02 1,20E-02 4,17E-03 0 2,18E-03 0,00E+00 2,55E-02 -5,24E-03
RWD kg 5,29E-06 2,72E-07 7,33E-07 2,61E-06 0,00E+00 0 3,05E-07 0,00E+00 4,41E-08 -3,64E-07
HWD = Hazardous waste disposed; NHWD = Non-hazardous waste disposed; RWD = Radioactive waste disposed
"Reading example: 9,0 E-03 = 9,0*10-3 = 0,009"
*INA Indicator Not Assessed
End of life - Output flow
Indicator Unit A1 A2 A3 A4 A5 C1 C2 C3 C4 D
CRU kg 0,00E+00 0,00E+00 0,00E+00 0,00E+00 0,00E+00 0 0,00E+00 0,00E+00 0,00E+00 0,00E+00
MFR kg 0,00E+00 0,00E+00 2,09E-02 0,00E+00 3,87E-03 0 0,00E+00 1,25E-02 1,65E-06 -9,60E-05
MER kg 0,00E+00 0,00E+00 3,93E-03 0,00E+00 2,49E-04 0 0,00E+00 1,84E-02 4,04E-08 -1,23E-05
EEE MJ 0,00E+00 0,00E+00 5,97E-03 0,00E+00 2,38E-04 0 0,00E+00 2,83E-02 2,62E-06 -4,51E-05
EET MJ 0,00E+00 0,00E+00 9,03E-02 0,00E+00 3,60E-03 0 0,00E+00 4,28E-01 3,97E-05 -6,82E-04
CRU = Components for re-use; MFR = Materials for recycling; MER = Materials for energy recovery; EEE = Exported energy electrical; EET = Exported energy thermal
"Reading example: 9,0 E-03 = 9,0*10-3 = 0,009"
*INA Indicator Not Assessed
Biogenic Carbon Content
Indicator Unit At the factory gate
Biogenic carbon content in product kg C 0,00E+00
Biogenic carbon content in accompanying packaging kg C 1,98E-03
Note: 1 kg biogenic carbon is equivalent to 44/12 kg CO2
10 / 12
Additional requirements
Greenhouse gas emissions from the use of electricity in the manufacturing phase
National production mix from import, low voltage (production of transmission lines, in addition to direct emissions and losses in grid) of applied
electricity for the manufacturing process (A3).
Electricity mix Source Amount Unit
Electricity, China (kWh) ecoinvent 3.6 1102,91 g CO2-eq/kWh
Dangerous substances
The product contains no substances given by the REACH Candidate list.
Indoor environment
No effect on indoor environment.
Additional Environmental Information
Additional environmental impact indicators required in NPCR Part A for construction products
Indicator Unit A1 A2 A3 A4 A5 C1 C2 C3 C4 D
GWPIOBC kg CO2 -eq 4,85E-01 2,81E-03 1,32E-01 2,70E-02 6,74E-05 0 2,97E-03 4,36E-02 2,28E-03 -1,07E-02
GWP-IOBC: Global warming potential calculated according to the principle of instantaneous oxidation. In order to increase the transparency of biogenic carbon​
contribution to climate impact, the indicator GWP-IOBC is required as it declares climate impacts calculated according to the principle of instantaneous oxidation.​
GWP-IOBC is also referred to as GWP-GHG in context to Swedish public procurement legislation.
11 / 12
Bibliography
ISO 14025:2010. Environmental labels and declarations - Type III environmental declarations - Principles and procedures. International
Organization for Standardization.
ISO 14044:2006. Environmental management - Life cycle assessment - Requirements and guidelines. International Organization for
Standardization.
EN 15804:2012+A2:2019. Environmental product declaration - Core rules for the product category of construction products. European
Committee for Standardization.
ISO 21930:2017. Sustainability in buildings and civil engineering works - Core rules for environmental product declarations of construction
products. International Organization for Standardization.
EN 50693:2019. Product category rules for life cycle assessments of electronic and electrical products and systems. European Committee for
Standardization.
Ecoinvent v3, 2019. Allocation, cut-off by classification. Swiss Centre of Life Cycle Inventories.
Iversen et al., (2021). eEPD v2021.09, background information for EPD generator tool system verification, LCA.no. Report number: 07.21. System
verification report.
Babwah & Philis (2023). EPD generator based on PCR EPD Italy 007, background information for EPD generator application and LCA data, LCA.no.
Report number 09.2023. PCR verification report (based on core PCR).
EPD Italy (2020). PCR EPD Italy 007 Part A for electronic and electrical products and systems. EPD Italy. Version 3, issue 13-01-2023 and valid
until 19-01-2025.
Program operator and publisher Phone: +47 977 22 020
The Norwegian EPD Foundation e-mail: post@epd-norge.no
Post Box 5250 Majorstuen, 0303 Oslo, Norway web: www.epd-norge.no
Owner of the declaration: Phone: +47 90021243
SG Armaturen AS e-mail: audun.skare@sg-as.no
Skytterheia 25, 4790 Lillesand, Norway web: www.sg-as.com
Author of the Life Cycle Assessment Phone: +47 916 50 916
LCA.no AS e-mail: post@lca.no
Dokka 6A, 1671 Kråkerøy, Norway web: www.lca.no
Developer of EPD generator Phone: +47 916 50 916
LCA.no AS e-mail: post@lca.no
Dokka 6A, 1671 Kråkerøy, Norway web: www.lca.no
ECO Platform web: www.eco-platform.org
ECO Portal web: ECO Portal
12 / 12
