Environmental Product
Declaration
as per ISO 14025 and EN 15804
Owner of the declaration: Holcon GmbH
Publisher: Kiwa-Ecobility Experts
Programme operator: Kiwa-Ecobility Experts
Declaration number: EPD-Holcon-157-EN (Rev.1_26.04.2023)
Issue date: 17-12-2021
Valid to: 16-12-2026
Precast concrete elements for
walls, pillars and beams
Based on the concrete recipe type 5
1. General information
Holcon GmbH Precast concrete
Programme operator Owner of the declaration
Kiwa-Ecobility Experts Holcon GmbH
Kiwa GmbH (formerly STF Holterman GmbH)
Voltastr. 5 Trajanring 25
13355 Berlin 46509 Xanten
Germany Germany
Declaration number Declared product / declared unit
EPD-Holcon-157-EN (Rev.1_26.04.2023) 1 m³ of precast concrete
This declaration is based on the Product Scope
Category Rules The average EPD (type: Cradle to gate with
PCR B - Product Category Rules for concrete modules C1–C4 and module D) is about cus-
and concrete elements; German version tom made precast concrete based on the con-
EN 16757:2017 crete recipe type 5, manufactured in Xanten,
Germany. The calculation is based on 1 m³ of
Issue date concrete with a share of 6 m% reinforcing and
17.12.2021 prestressed steel.
Kiwa-Ecobility Experts shall not be liable with
Valid to respect to manufacturer information, life cy-
16.12.2026 cle assessment data and evidences.
Verification
The standard EN 15804+A2:2019 serves as the
core PCR
Independent verification of the declaration
and data according to ISO 14025:2011-10
☐internally ☒externally
Frank Huppertz
(Head of Kiwa-Ecobility Experts)
Prof. Dr. Frank Heimbecher Max Sonnen
(Chairman of the independent expert committee - (External verifier – Ecomatters)
Ecobility Experts)
Page | 2 Holcon - precast concrete elements based on type 5
2. Product
2.1 Product description
The products are reinforced and prestressed precast concrete elements in various formats, sizes and
applications. The elements are used as columns, walls and beams. The concrete type 5 has compressive
strength class of C 55/67.
2.2 Application
The products are prefabricated elements for building, civil engineering and bridge construction, balco-
nies, solid ceilings.
2.3 Placing on the market / Application rules
• EN 1168 Precast concrete products - Hollow core slabs
• EN 13224 Ribbed floor elements
• EN 13225 Precast concrete products - Linear structural elements
• EN 14992 Precast concrete products - Wall elements
2.4 Technical Data
Technical Data – Concrete type 5
Name Value Unit
Compressive strength C 55/67 -
Target value of the initial test (28 d) 71 N/mm²
Consistency class F6(>630) -
Maximum w/c ratio 0,45 -
Maximum aggregate size (D ) 16 mm
max
Air content 1,6 %
Workability time 0,5 h
Steel grade B500B and B500A -
2.5 Base materials / Ancillary
Name Value Unit
Cement 15 m%
Aggregates 69 m%
Addition (lime) 9 m%
Water 7 m%
Admixture <1 m%
Steel 6 m%
There is no biogenic carbon in the product.
2.6 Manufacturing
The manufacturing contains the following processes:
• Delivery of raw materials
• Preparation of the moulds (formwork, cutting and laying of the probation steel elements,
placeholders)
• Concrete mixing and filling into the mould, curing
• Removal of the formwork, finishing, storage
Page | 3 Holcon - precast concrete elements based on type 5
Figure 1: Overview about the production route precast concrete (A1 - A3, C1-C4, D)
2.7 Packaging
No packaging materials are used.
2.8 Production waste
The production process generates production residues and waste: Metal scrap and scale and ancillary
materials (lubricating oil, electrode copper).
Page | 4 Holcon - precast concrete elements based on type 5
3. LCA: Calculation rules
3.1 Declared unit
The EPD refers to the declared the product system of 1 cubic meter precast concrete.
Name Value Unit
Declared unit 1 m3 Concrete Element
Weight per Unit: 2.407,5 kg
Compressive strength class C55/67 -
Content of reinforcing steel 6 m%
and precast steel
Steel grade B500B / B500A -
3.2 System boundary
This EPD was created in accordance with EN 15804 and monitors the production stage and the end-of-
life stage. According to EN 15804 this corresponds to product phases A1-A3, C1-C4 and D (EPD type
"Cradle to gate with modules C1–C4 and module D”). All inputs including raw materials, primary prod-
ucts, energy and auxiliary materials as well as the accumulated waste are considered in the assess-
ment. The installation and the use of the final product is not within the manufacturer's sphere of in-
fluence. Therefore, modules A4, A5 and B1-7 have not been considered. The effect of CO absorption
2
through the carbonization process is not taken into account in the LCA. The reference year is 2020. The
geographical reference area is Germany.
3.3 Estimates and assumptions
The average proportion of prestressing steel at the Xanten site (type 5) is 14 kg of steel.
Modules B1 to B7: For concrete components, maintenance and repair measures are generally not nec-
essary during the reference service life, so that no environmental burdens arise in these modules. In
addition, no energy or water is consumed.
3.4 Cut-off criteria
All material flows that contribute to more than 1% of the total mass, energy or environmental impact
of the system have been considered in the LCA. It can be assumed that the neglected processes in total
contributed less than 5% to the considered impact categories.
The production of the machines, plants and other infrastructure required to produce the reinforce-
ment steel products were not taken into account in the LCA.
3.5 Background Data
The background data is taken from Ecoinvent database version 3.6. The life cycle assessment was mod-
eled with the NIBE tool. Geographical reference space of the background data is Germany. Almost all
consistent datasets contained in the Ecoinvent database are documented and can be viewed in the
online Ecoinvent documentation.
3.6 Data quality
Overall, the quality of the data can be considered as good. In the operating data survey all relevant
process-specific data could be collected. The data relating to the manufacturing phase of the construc-
tion steel are determined by Holcon and refers to the production site in Xanten.
The LCA study by STF Holterman Wapeninsstaal BV (Tauw 2020) provides primary data (steel produc-
tion, transport, processing) on the probationary steel used, which was integrated in this study. As the
Page | 5 Holcon - precast concrete elements based on type 5
LCA study uses the calculation method EN15804+A1, the LCA results could not be used. In the LCI, the
data used for the calculation of the semi-finished product reinforcing steel are also listed.
Secondary data were taken from the Ecoinvent 3.6 database. The database is regularly checked and
thus complies with the requirements of ISO 14040/44 (background data not older than 10 years). The
background data meets the requirements of EN 15804. The quantities of raw materials, consumables
and supplies used as well as the energy consumption have been recorded and averaged over the entire
year of operation.
The general rule has been that specific data from specific production processes or average data derived
from specific processes must be given priority when calculating an EPD or Life Cycle Assessment. Data
for processes that the manufacturer cannot influence or choose, were backed up with generic data.
EPDs of raw materials (Cement) were partly available but not usable, as they were calculated according
to EN 15804:2014 (+A1) and not according to the EN 15804:2020 (+A2) standard used here.
3.7 Period Under review
All process-specific data was collected for the operating year 2020. The quantities of raw and auxiliary
materials as well as energy consumption have been recorded and averaged over the entire operating
year 2020.
3.8 Allocation
There are no co-products in the raw material supply phase, so no allocation methods were used at this
stage. There are no allocations during the manufacturing phase at the plant. The preparation of the
construction product is an independent process.
3.9 Calculation methods
For life cycle assessment, the calculation methods described in ISO 14040 have been applied. The eval-
uation is based on the phases in the system boundaries.
3.10 Mix of electricity and CO -Certificates
2
The electricity mix was chosen according to the energy grid mix in Germany (reference year 2018). No
CO certificates were counted.
2
3.11 Comparability
Basically, a comparison or an evaluation of EPD data is only possible if all the data sets to be compared
were created according to EN 15804 and the building context, respectively the product-specific char-
acteristics of performance, are considered.
3.12 Reference Service Life (RSL)
The lifetime of reinforcement will be limited by the service life of the construction. The concrete com-
position limits given in EN 206-1 are specified for an intended service life of at least 50 years under the
respective exposure classes/ environmental conditions.
Page | 6 Holcon - precast concrete elements based on type 5
4. LCA: Scenarios and additional technical information
C1 Demolition: According to the current state of the art, the demolition of concrete and reinforced
concrete structures is mainly carried out with longfront excavators equipped with demolition clamps.
The concrete buildings are demolished by so-called "press cutting", i.e. the crushing of concrete by
applying a compressive force. It is estimated that one site vehicle is in operation for 30 minutes per
sqm of concrete element (conservative assumption).
C2 - C4 and D: It is assumed that concrete and reinforcement material are separated after deconstruc-
tion. For both waste groups, a waste scenario according to the Dutch National Environmental Database
(NMD) (SBK 2019) is applied:
• Concrete (i.a. elements, brickwork): 99% of concrete is recycled and reused as aggregate.
• Steel, reinforcement: 95% of reinforcing steel is marketed as scrap metal.
5. LCA: Results
The following tables show the results of the impact assessment indicators, resource use, waste and
other output streams. The results presented here refer to the declared average product.
Page | 7 Holcon - precast concrete elements based on type 5
Description of the system boundary
Benefits and
Construction loads beyond
Product stage Use stage End of life stage
process stage the system
boundaries
y lp p u s la ir e t a m w a R t r o p s n a r T g n ir u t c a fu n a M m o r f t r o pu s nn aa rm T-e s u fo e c a lp o t r e r u t c a f n on io t cit ua rl tl sa nts on C-is s e c o r p e s U e c n a n e tn ia M r ia p e R tn e m e c a lp e R n e m h s ib r u fe R e s u y g r e n e la n o it a r e p O e s u r e t a w la n o it a r e p O / n o it c u r ts n eo Dc -n o itilo m e d t r o p s n a r T g n is s e c o r p e ts a W la s o p s iD y r e v eo s uc ee RR -- ga ni it ln c ye ct o e Rp -l
A1 A2 A3 A4 A5 B1 B2 B3 B4 B5 B6 B7 C1 C2 C3 C4 D
X X X MND MND MND MND MND MND MND MND MND X X X X X
X=Module declared | MND=Module not declared
Results of the LCA – Environmental impact: 1m³ of concrete type 5
Parameter Unit A1 A2 A3 C1 C2 C3 C4 D Total
Core environmental impact indicators (EN 15804)
ADP-mm kg Sb-eqv. 4,04E-03 9,01E-04 1,85E-04 8,03E-05 8,05E-04 2,17E-05 2,76E-06 -1,06E-03 7,48E-03
ADP-f MJ 5,52E+03 5,36E+02 9,50E+02 7,21E+02 4,79E+02 1,04E+02 8,42E+00 -5,51E+02 9,35E+03
AP mol H+ eqv. 2,62E+00 2,06E-01 1,72E-01 5,48E-01 1,84E-01 4,84E-02 2,86E-03 -3,21E-01 4,07E+00
EP-fw kg P eqv. 1,90E-02 3,59E-04 5,90E-03 1,91E-04 3,20E-04 2,40E-04 3,38E-06 -2,31E-03 2,52E-02
EP-m kg N eqv. 6,31E-01 7,26E-02 5,14E-02 2,42E-01 6,49E-02 1,93E-02 9,84E-04 -7,51E-02 1,22E+00
EP-T mol N eqv. 7,34E+00 8,01E-01 5,48E-01 2,65E+00 7,15E-01 2,14E-01 1,08E-02 -8,73E-01 1,38E+01
GWP-b kg CO2 eqv. 1,10E+01 1,64E-02 3,05E+00 1,46E-02 1,47E-02 4,46E-02 5,97E-04 4,56E-01 1,51E+01
GWP-f kg CO2 eqv. 8,59E+02 3,55E+01 6,96E+01 5,24E+01 3,18E+01 7,71E+00 3,01E-01 -6,84E+01 1,11E+03
GWP-luluc kg CO2 eqv. 2,86E-01 1,30E-02 4,52E-02 4,13E-03 1,16E-02 1,47E-03 8,40E-05 2,48E-02 4,27E-01
GWP-total kg CO2 eqv. 8,70E+02 3,56E+01 7,27E+01 5,24E+01 3,18E+01 7,76E+00 3,02E-01 -6,79E+01 1,12E+03
kg CFC 11
ODP 4,01E-05 7,85E-06 5,88E-06 1,13E-05 7,01E-06 1,00E-06 1,24E-07 -2,94E-06 9,25E-05
eqv.
kg NMVOC
POCP 2,24E+00 2,29E-01 1,32E-01 7,30E-01 2,04E-01 5,81E-02 3,15E-03 -4,12E-01 3,85E+00
eqv.
m3 world
WDP 2,92E+02 1,92E+00 2,73E+00 9,66E-01 1,71E+00 4,69E-01 3,78E-01 -3,04E+02 7,11E+00
eqv.
Additional environmental impact indicators (EN 15804)
ETP-fw CTUe 1,06E+04 4,78E+02 6,23E+02 4,35E+02 4,27E+02 8,40E+01 5,46E+00 -2,04E+03 1,21E+04
HTP-c CTUh 2,03E-06 1,55E-08 1,56E-08 1,52E-08 1,39E-08 1,99E-09 1,26E-10 4,43E-08 2,19E-06
HTP-nc CTUh 5,06E-05 5,23E-07 5,00E-07 3,73E-07 4,67E-07 5,63E-08 3,88E-09 1,17E-05 6,59E-05
kBq U235
IR 2,28E+01 2,25E+00 2,09E+00 3,09E+00 2,01E+00 3,28E-01 3,46E-02 1,25E-01 3,92E+01
eqv.
disease in-
PM 2,85E-05 3,20E-06 1,56E-06 1,45E-05 2,86E-06 1,07E-06 5,56E-08 -4,98E-06 5,59E-05
cidence
SQP Pt 1,75E+03 4,65E+02 1,21E+02 9,20E+01 4,15E+02 1,73E+01 1,77E+01 -3,97E+02 3,76E+03
ADP-mm=Depletion of abiotic resources- minerals and metal| ADP-f=Depletion of abiotic resources - fossil fuels | AP=Acidification of soil
and water | EP-fw =Eutrophication, freshwater | EP-m=Eutrophication marine | EP-T=Eutrophication, terrestrial | GWP-b=Global warming
potential - Biogenic | GWP-f=Global warming potential - Fossil | GWP-luluc=Global warming potential - Land use and land use change
|GWP-total=Global warming potential |ODP=Ozone layer depletion |POCP=Photochemical oxidants creation | WDP=Water use | ETP-
fw=Ecotoxicity, freshwater | HTP-c=Human toxicity, cancer | HTP-nc=Human toxicity, non-cancer | IR=Ionising radiation, human health |
PM=Particulate Matter | SQP=Land use
Page | 8 Holcon - precast concrete elements based on type 5
Disclaimer on ADP-mm, ADP-f, WDP, ETP-fw, HTP-c, HTP-nc, SQP: The results of these environmental
impact indicators must be used with caution, as the uncertainties in these results are high or as there
is limited experience with the indicator.
Disclaimer on IR: This impact category mainly addresses the potential effect of low dose ionizing radi-
ation on human health in the nuclear fuel cycle. It does not consider effects due to possible nuclear
accidents and occupational exposures, nor does it consider radioactive waste disposal in underground
facilities. Potential ionizing radiation from soil, radon, and some building materials is also not measured
by this indicator.
Resource use and environmental information: 1m³ of concrete type 5
Parameter Unit A1 A2 A3 C1 C2 C3 C4 D Total
PERE MJ 3,92E+02 6,71E+00 6,35E+01 3,90E+00 6,00E+00 5,89E+00 6,81E-02 -3,10E+00 4,75E+02
PERM MJ 0,00E+00 0,00E+00 2,39E-01 0,00E+00 0,00E+00 0,00E+00 0,00E+00 -3,78E-04 2,39E-01
PERT MJ 3,92E+02 6,71E+00 6,37E+01 3,90E+00 6,00E+00 5,89E+00 6,81E-02 -3,10E+00 4,75E+02
PENRE MJ 5,85E+03 5,69E+02 1,03E+03 7,66E+02 5,08E+02 1,10E+02 8,95E+00 -5,76E+02 8,27E+03
PENRM MJ 0,00E+00 0,00E+00 0,00E+00 0,00E+00 0,00E+00 0,00E+00 0,00E+00 0,00E+00 0,00E+00
PENRT MJ 5,85E+03 5,69E+02 1,03E+03 7,66E+02 5,08E+02 1,10E+02 8,95E+00 -5,76E+02 8,27E+03
SM Kg 1,43E+02 0,00E+00 8,27E-02 0,00E+00 0,00E+00 0,00E+00 0,00E+00 0,00E+00 1,43E+02
RSF MJ 0,00E+00 0,00E+00 0,00E+00 0,00E+00 0,00E+00 0,00E+00 0,00E+00 0,00E+00 0,00E+00
NRSF MJ 0,00E+00 0,00E+00 0,00E+00 0,00E+00 0,00E+00 0,00E+00 0,00E+00 0,00E+00 0,00E+00
FW m3 9,57E+00 6,53E-02 2,66E-01 3,71E-02 5,83E-02 3,46E-02 9,00E-03 -7,08E+00 2,96E+00
HWD Kg 1,35E-02 1,36E-03 8,77E-04 1,96E-03 1,21E-03 1,80E-04 1,26E-05 -6,49E-03 1,27E-02
NHWD Kg 7,04E+01 3,40E+01 3,85E+00 8,54E-01 3,04E+01 1,44E+01 5,72E+01 -8,17E+00 2,03E+02
RWD Kg 2,44E-02 3,52E-03 2,76E-03 5,01E-03 3,14E-03 4,65E-04 5,53E-05 -6,03E-04 3,87E-02
CRU Kg 0,00E+00 0,00E+00 0,00E+00 0,00E+00 0,00E+00 0,00E+00 0,00E+00 0,00E+00 0,00E+00
MFR Kg 0,00E+00 0,00E+00 4,77E+01 0,00E+00 0,00E+00 4,92E+03 0,00E+00 0,00E+00 4,96E+03
MER Kg 0,00E+00 0,00E+00 0,00E+00 0,00E+00 0,00E+00 0,00E+00 0,00E+00 0,00E+00 0,00E+00
EE MJ 0,00E+00 0,00E+00 1,05E-01 0,00E+00 0,00E+00 0,00E+00 0,00E+00 3,15E-03 1,08E-01
EET MJ 0,00E+00 0,00E+00 6,64E-02 0,00E+00 0,00E+00 0,00E+00 0,00E+00 1,99E-03 6,83E-02
EEE MJ 0,00E+00 0,00E+00 3,85E-02 0,00E+00 0,00E+00 0,00E+00 0,00E+00 1,16E-03 3,97E-02
PERE=renewable primary energy ex. raw materials | PERM=renewable primary energy used as raw materials | PERT=renewable primary
energy total | PENRE=non-renewable primary energy ex. raw materials | PENRM=non-renewable primary energy used as raw materials |
PENRT=non-renewable primary energy total | SM=use of secondary material | RSF=use of renewable secondary fuels | NRSF=use of non-
renewable secondary fuels | FW=use of net fresh water | HWD=hazardous waste disposed | NHWD=non-hazardous waste disposed |
RWD=radioactive waste disposed | CRU=Components for re-use | MFR=Materials for recycling | MER=Materials for energy recovery |
EE=Exported energy | EET=Exported Energy Thermic | EEE=Exported Energy Electric
Page | 9 Holcon - precast concrete elements based on type 5
6. LCA: Interpretation
The following figures shows the influence of the different life stages on the environmental core indi-
cators for concrete type 5. Since the Global Warming Potential biogen (GWP-b) and Global Warming
Potential resulting from land use and land use (GWP-luluc) change have only a minor impact, only total
Global Warming Potential (GWP-total) is displayed. As shown in Figure 1 the majority of the environ-
mental impact is attributed to row material processing phase (A1), followed by the transports of raw
materials (A2) and production (A3).
100%
80%
60%
40%
20%
0%
-20%
-40%
-60%
ADP-mm ADP-f AP EP-fw EP-m EP-T GWP-total ODP POCP WDP
A1 A2 A3 C1 C2 C3 C4 D
Figure 1: Influence of the modules on the environmental core indicators for type 5
Overall, the quality of the data can be considered as good. In the operating data survey all relevant
process-specific data could be collected. The data relating to the manufacturing phase of the precast
concrete are determined by Holcon and refers to the production site in Xanten (Germany).
Secondary data were taken from the Ecoinvent 3.6 database. The database is regularly checked and
thus complies with the requirements of ISO 14040/44 (background data not old-er than 10 years). The
background data meets the requirements of EN 15804. The quantities of raw materials, consumables
and supplies used as well as the energy consumption have been recorded and averaged over the entire
year of operation.
EPDs of raw materials could not be used because they were still calculated according to the old stand-
ard (EN 15804+A1), therefore secondary data had to be used. As all reinforcing steel products (except
prestressing steel) were supplied by the steel processor Holterman Wapeningsstaal BV, accurate data
on the production process as well as the origin of the steel could be used.
Data quality was calculated using the Data Quality Rating method according to the PEF approach. The
DQRs range from 1,75 to 2,25 for the most abundant inputs in terms of mass. The expenses for dis-
mantling (C1) could only be estimated, which is why the DQR value here is 3.0. However, the impact
of the module on the overall Life Cycle Assessment is very low.
Page | 10 Holcon - precast concrete elements based on type 5
7. References
European Commission Joint Research Centre Institute for Prospective Technological Studies (JCR
2014): End-of-waste criteria for waste plastic for conversion, Seville, 2014, doi:10.2791/13033
CML-IA April 2013 – Characterisation factors developed by Institute of Environmental Sci-ences (CML):
University Leiden (NL)- http://www.cml.leiden.edu/software/data-cmlia.html
Klöpffer, W., Grahl B.: Ökobilanz (LCA) – Ein Leitfaden für die Ausbildung und Beruf, Wily-VCH Verlag
GmbH&Co.KgaA, Weinheim (DE), 2007
Protocol EPD-online - 25011.16.03.015 - Protocol EPD online - NMD, version 1.2, November 2016, NIBE
Stichting Bouwkwaliteit (SBK 2019): Assessment Method - Environmental Performance Con-struction
and Civil Engineering Works (GWW), Rijswijk, Version "3.0 January 2019" incl. amendments July 2019,
Jan 2020
Stichting Bouwkwaliteit: verification protocol - inclusion data in the Dutch environmental data-base,
Rijswijk, Final Version 3.0, January 2019
TAUW 2020: LCA en MKI-berekening voor wapeningsstaal van Holterman Wapeningsstaal BV, TAUW
bv, Deventer (NL) October 2020,
Standards and laws
ISO 14040:2006-10, Environmental management - Life cycle assessment - Principles and framework;
EN ISO 14040:2006
ISO 14044:2006, Environmental management - Life cycle assessment - Requirements and guidelines;
EN ISO 14040:2006
ISO 14025:2011-10: Environmental labels and declarations — Type III environmental decla-rations —
Principles and procedures EN 13249
EN 15804:2014 (+A1): Sustainability of construction works — Environmental Product Decla-rations —
Core rules for the product category of construction products
EN 15804:2020 (+A2): Sustainability of construction works - Environmental product declara-tions -
Core rules for the product category of construction products
EN 16757:2017: Sustainability of construction works – Environmental product declarations – Product
Category Rules for concrete and concrete elements
Page | 11 Holcon - precast concrete elements based on type 5
Publisher Mail DE.Ecobility.Ex-
Kiwa - Ecobility Experts perts@kiwa.com
Kiwa GmbH Web https://www.kiwa.com/de/de
Voltastr.5, 13355 Berlin /uber-kiwa/ecobility-experts/
Germany
Programme operator Mail DE.Ecobility.Ex-
Kiwa - Ecobility Experts perts@kiwa.com
Kiwa GmbH Web https://www.kiwa.com/de/de
Voltastr.5, 13355 Berlin /uber-kiwa/ecobility-experts/
Germany
Author of the Life Cycle Tel. +49 (0)30 467761-43
Assessment Fax. +49 (0)30 467761-10
Kiwa GmbH Mail DE.Nachhaltigkeit@kiwa.com
Voltastr.5, 13355 Berlin Web https://www.kiwa.com/
Germany
Owner of the declaration Tel. +49 (0)28 01984420
Holcon GmbH Fax. +49 (0)28 019844229
Trajanring 25 Mail info@holcon.de
46509 Xanten Web https://holcon.de/
Germany
Kiwa-Ecobility Experts -
established member of
Page | 12 Holcon - precast concrete elements based on type 5
