ENVIRONMENTAL PRODUCT DECLARATION
as per ISO 14025 and EN 15804+A2
Owner of the Declaration Etex Building Performance International
Publisher Institut Bauen und Umwelt e.V. (IBU)
Programme holder Institut Bauen und Umwelt e.V. (IBU)
Declaration number EPD-ETE-20240003-IBC1-EN
Issue date 12.03.2024
Valid to 11.03.2029
PregyMetal - Z100 galvanized steel profiles 1mm thickness
Etex Building Performance SpA
www.ibu-epd.com | https://epd-online.com
1. General Information
Etex Building Performance SpA PregyMetal - Z100 galvanized steel profiles 1mm
thickness
Programme holder Owner of the declaration
IBU – Institut Bauen und Umwelt e.V. Etex Building Performance International
Hegelplatz 1 Rue Marcel Demonque 500
10117 Berlin 84915 Avignon Cedex 9
Germany France
Declaration number Declared product / declared unit
EPD-ETE-20240003-IBC1-EN 1 kg of average steel structure for PregyMetal profile with z100
galvanization and 1 mm thickness.
This declaration is based on the product category rules: Scope:
Structural steels, 01.08.2021 This EPD is an average EPD and applies for the following specific SINIAT
(PCR checked and approved by the SVR) produts brand developed by Etex Building Performace S.p.A: Montante
PregyMetal C75-50x1, Montante PregyMetal C100-50x1, Montante
PregyMetal C150-50x1.
Issue date This EPD was developed from data collected at the Etex Building
Performace S.p.A steel profile factory located in Corfinio. CAP 67030 (AQ),
12.03.2024
Italy, producing 100% of the total production of these products. Data refers
to year 2021.
The EPD is a cradle-to-gate with options EPD and covers Siniat
Valid to
PregyMetal steel profiles with 1mm thickness.
11.03.2029
The owner of the declaration shall be liable for the underlying information
and evidence; the IBU shall not be liable with respect to manufacturer
information, life cycle assessment data and evidences.
The EPD was created according to the specifications of EN 15804+A2. In
the following, the standard will be simplified as EN 15804.
Verification
The standard EN 15804 serves as the core PCR
Independent verification of the declaration and data according to ISO
Dipl.-Ing. Hans Peters
14025:2011
(Chairman of Institut Bauen und Umwelt e.V.)
internally X externally
Florian Pronold Vito D'Incognito,
(Managing Director Institut Bauen und Umwelt e.V.) (Independent verifier)
1 Environmental Product Declaration - Etex Building Performance SpA - PregyMetal - Z100 galvanized steel profiles 1mm thickness
2. Product
slats.
2.1 Product description/Product definition
Siniat PregyMetal profiles covered by this EPD are used in the 2.5 Base materials/Ancillary materials
construction sector as a support framing for plasterboard walls:
Steel profile
- 'C' studs Montanti sp.1mm, reinforced profiles that constitute
Name Value Unit
the vertical structures of the wall frames.
The galvanized carbon steel profiles here studied have a Z100 Galvanized carbon steel DX51D 1 Kg
zinc coating (100 g/m2 as minimum weight), mainly used for Recycled steel content 35 %
internal walls and counter-walls.
Siniat PregyMetal profiles covered by this EPD are made from
The EPD covers the Italian version of the steel profiles for
galvanized carbon steel DX51D with 35% of post consumer
plasterboard drywall systems.
recycled content.
The EPD refers to 1 average kg of steel profiles with coating
The metallic coating is the Z100 zinc coating where the
and 1mm thickness. For the placing on the market of the
galvanization is made of zinc for > 99% and is characterized by
product in the European Union/European Free Trade
100 g/m2 on both sides.
Association (EU/EFTA) (with the exception of Switzerland)
The steel profiles covered by this EPD do not contain any
Regulation (EU) No. 305/2011 (CPR) applies. The product
substances listed in the 'Candidate List of Substances of Very
needs a declaration of performance taking into consideration
High Concern for Authorisation' (SVHC)
EN 14195:2005, Metal framing components for gypsum board
/(https://echa.europa.eu/it/candidate-list-table - date:
systems - Definitions, requirements and test methods and the
27.06.2018)/ exceeding 0.1% by mass.
CE-marking.
For the application and use the respective national provisions
The Candidate list can be found on the ECHA website address:
apply.
https://echa.europa.eu/de/home.
2.2 Application
The steel profiles covered by this EPD do not contain any other
Siniat PregyMetal profiles covered by this EPD are used in all
carcinogenic, mutagenic, reprotoxic (CMR) substances in
construction types (residential, commercial, healthcare, ...new
categories 1A or 1B which are not on the candidate list,
or renovation), to build drywall systems. The various profiles
exceeding 0.1% by mass.
can be used as vertical plasterboard frames, with improved
stiffness and mechanical properties for high walls. They can be
2.6 Manufacture
considered easy to install products.
The manufacturing process is illustrated in the Figure below.
Possible plasterboard frames fields of application are for interior
use, for walls and ceilings.
The production process consists of cutting, modeling, and
2.3 Technical Data drilling of channels, studs and metal tracks. The raw materials
first arrive at the plants in the form of rolls of galvanized steel,
Detailed technical information is available in the specific
separated from each other by wooden slats, bound by plastic
product data sheets at www.siniat.it.
straps and subsequently stored inside the Company's
warehouse. The actual process begins when the rolls of raw
- Performance data of the product in accordance with the
material are placed at the beginning of special machines that
declaration of performance with respect to its essential
work the profiles. Initially, the steel coil is unrolled and passes
characteristics according to UNI EN 14195:2005
through a set of rollers that gives the desired shape (U or C).
Subsequently, the profile thus formed passes through a
- Tensile strenght: ≥ 300 N/mm2
machine that drills it according to pre-established schemes.
Finally, the formed and perforated steel structures are cut in
- Quality steel grade: DX51 D+Z100
length according to predetermined measures. The finished
products are then grouped and held together by plastic
- Class of reaction to fire performance: A1
strapping and separated from each other with wooden slats.
The management system operated by the site is in compliance
Constructional data with the UNI EN ISO 9001:2015.
Below is a list of the number of meters necessary to obtain 1 kg
of each individual product (o profile)
Name Value Unit
Density 7.85 kg/m3
Montante PregyMetal C75/50x1 0.71 m
Montante PregyMetal C100/50x1 0.62 m
Montante PregyMetal C150/50x1 0.57 m
Performance data of the product in accordance with the
declaration of performance with respect to its essential
characteristics according to UNI EN 14195:2005
2.4 Delivery status
Siniat PregyMetal profiles covered by this EPD are delivered in
variable dimensions, specified by their respective data sheets
available at www.siniat.it. The typical length of the structures is
3 m. The selling unit is a set of a defined number of structures
bound by different plastic straps and separated by wooden 2.7 Environment and health during manufacturing
2 Environmental Product Declaration - Etex Building Performance SpA - PregyMetal - Z100 galvanized steel profiles 1mm thickness
Relating to health protection during the manufacturing process, substitutions. In this particular case, in accordance with the
the plant follows and respects the specific Italian Regulation. "Federal office for building an regional planning" BBSR table
The manufacturing process is certified according to "Service lives of components for life cycle assessment
Occupational Health and Safety Management System UNI ISO according to BNB" (http://www.nachhaltigesbauen.de/baustoff-
45001:2018. und-gebaeudedaten/nutzungsdauern-von-bauteilen.html), a
Steel profiles are manufactured in a plant permitted by emission service life can be declared (not a RSL according to ISO
law and by external waste recovery in accordance with the 15686). The voice 'Unterkonstruktionen: Trockenbauprofile
Italian regulation. The management system operated by the site (Stahl, Holz)', meaning Drywall profiles for substructures, here
is in compliance with the standard UNI EN ISO 14001:2015. in steel. The service life is considered to be higher than 50
years.
2.8 Product processing/Installation Description of the influences on the ageing of the product when
The manufacturing process is carried out in dedicated applied in accordance with the rules of technology.
automated machines that work the profiles: security protections
according to the safety machinery standards are installed to
avoid any risks for operators. 2.13 Extraordinary effects
During handling, storage and installation: eye protection should Fire
be worn when using hand tools, gloves should be worn when Information on the fire performance according to EN 13501:1 or
handling metal sections and components to avoid risk of established national standards. According to EN 13501:1:
lacerations, packs should be stacked in a safe and stable
manner, pack strapping should not be used for lifting, coils and - The classes of building products regarding their fire
metal sections may spring apart when strapping is released. performance are predefined as: A1
Water
2.9 Packaging Contains no substances that have any impact on water in case
For product protection the steel profiles are packed in groups of of flood.
192 or 360 and held together with plastic strapping and wooden
slats. Mechanical destruction
If relevant: information on the product performance including
2.10 Condition of use
possible impacts on the environment following unforeseeable
Siniat PregyMetal profiles for plasterboard are suitable for any mechanical destruction.
type of wall and ceiling created for plasterboard systems. No
maintenance or repair is required over the service life. The
material composition of the product does not change during its 2.14 Re-use phase
use phase. For the "C3" recycling phase, a scenario was used that
recovers 90% of the steel and therefore sent for material
2.11 Environment and health during use
recovery
These products are not classified as hazardous under the EU
CLP Regulation (European Regulation EC/1272/2008 on the 2.15 Disposal
classification, labelling and packaging of substances and Disposal in accordance with the waste code: 17 04 05 Steel
mixtures). and iron waste from construction and demolition operations.
The structures can be dissembled and, since they are entirely
2.12 Reference service life
made out of steel, at least 90% can be recycled.
The reference service life (RSL) is not relevant for National disposal guidelines have to be observed.
consideration of the LCA as the steel structures are long-lasting
products, therefore the use phase is not considered. 2.16 Further information
Furthermore, the use stage (modules B1-B7) doesn't cause any www.siniat.it
environmental impact as the structures, once installed, do not
require any manufacturing, water or electricity use or
3. LCA: Calculation rules
3.1 Declared Unit
• steel structures manufacturing (modules A1-A3),
The LCA results presented in this EPD are related to 1 kg of
including the production of the steel rolls, the transport
average steel profile with 1mm thickness. The arithmetic mean
to the manufacturing site, as well as impacts due to
was carried out between the environmental impact results of
energy consumption, as well as auxiliary materials,
the different products considered.
waste treatment;
Declared unit and mass reference • transport of the steel structures from the manufacturing
Name Value Unit to the building site (module A4),
Installation (module A5), including the production of
Declared unit 1 kg
auxiliaries and of waste deriving from packaging;
Conversion factor:
• emissions during the use phase (modules B). No
Montante PregyMetal C75/50x1 0.71 m/kg
emissions occur during the Etex Building Performace
Montante PregyMetal C100/50x1 0.62 m/kg S.p.A steel structure use phase;
Montante PregyMetal C1150/50x1 0.57 m/kg • end-of-life (modules C1-C4), including impacts from
Density 7500 kg/m3 manual deconstruction, transport of waste to treatment
facility, and waste processing and waste disposal. The
scenario studied considers 90% of the structure
3.2 System boundary
recyclable (C3) and 10% sent to landfill (C4);
This EPD is a cradle-to-gate with options EPD, covering the
• benefits and loads beyond the system boundaries (D).
following life cycle stages:
3 Environmental Product Declaration - Etex Building Performance SpA - PregyMetal - Z100 galvanized steel profiles 1mm thickness
process remain identical.
3.3 Estimates and assumptions
Assumptions regarding transport distances were made for the 3.7 Period under review
installation and end-of-life of the studied products, following the The data used for the study complies with the current level of
indications found in the EN 15804+A2 standard. knowledge at the time of modelling the LCA in 2021.
3.4 Cut-off criteria 3.8 Geographic Representativeness
In this study the packaging relating to the packaging materials Land or region, in which the declared product system is
of the finished product were placed in Cut-Off. manufactured, used or handled at the end of the product´s
lifespan: EU-27 Member States
3.5 Background data
The life cycle model supporting the EPD was developed in
SimaPro 9.5, using background data from Ecoinvent 3.9.1, with 3.9 Allocation
the cutoff system model. When background data representative In accordance with the PCR, the allocation was made
of the Italian market was not available in the Ecoinvent considering the production of 2021. Specifically, the total
database, European average data ('Europe without Switzerland' quantity of profiles produced at the Corfinio plant, measured in
or 'RER') or global data ('GLO') was used instead. mass (kg), was obtained from the internal monitoring reports.
The percentages of the studied metal structures compared to
3.6 Data quality the total production within the Corfinio plant is 91%.
Background data is from the Ecoinvent 3.9.1 database. Some
of these background datasets have been collected more than 3.10 Comparability
10 years ago but are still representative of current technology. Basically, a comparison or an evaluation of EPD data is only
Primary data provided by Etex Building Performace S.p.A and possible if all the data sets to be compared were created
reviewed by Greenwich Srl is representative of the annual according to EN 15804 and the building context, respectively
production for the year 2021.Since this is an average EPD, the the product-specific characteristics of performance, are taken
environmental impacts reported are considered representative into account. Background data base : Ecoinvent 3.9.1
of all products as both the raw material and the production
4. LCA: Scenarios and additional technical information
The use stage (module B1-B7) have no impacts. The profiles
Characteristic product properties of biogenic carbon have a reference service life of 50 years according to Federal
The total mass of biogenic carbon containing materials is less office for building and regional planning (BBSR). The product
than 5 % of the total mass of the product and accompanying will last in situ with no requirements for maintenance, repair,
packaging. replacement or refurbishment throughout this period.
Note: 1 kg of biogenic carbon is equivalent to 44/12 kg of CO .
2 Reference service life
Name ValueUnit
The A5 installation phase considers all materials, waste and
energy consumed to install the studied product at the Life Span (according to BBSR) 50 a
construction site into the building. Maintenance e.g. required frequency, type and
- -
The steel structures that arrive on site are positioned manually quality and replacement of components
and installed using a drill to screw the screws to hold the
various structural parts (studs, tracks etc.) together, ready to End of life (C1 - C4)
contain the plasterboard wall or ceiling that will be placed there, C1:The product dismantling from the building is done manually
without the need for auxiliary materials. through the use of a drill to unscrew the screws that hold the
channels, studs and tracks together.
Installation into the building (A5)
C2: 100 km estimated
For the installation phase, a typical situation was estimated per
C3: 90% of product mass is recycled
meter of structure installed:
C4: 10% of product mass is send to landfill
- screws per meter = 10
Name Value Unit
- seconds needed to tighten a screw = 5
- Total operating time = 50 seconds Recycling 0.9 kg
- Drill power = 600W Landfilling 0.1 kg
A consumption of 0,0208 kWh of electricity is therefore
estimated for every meter of structure installed.
Name Value Unit
Electricity consumption 0.0208 kWh
4 Environmental Product Declaration - Etex Building Performance SpA - PregyMetal - Z100 galvanized steel profiles 1mm thickness
5. LCA: Results
The following table shows the result of the LCA for 1 kg of the reference product. The results in the B module are based on a period of
one year as no reference service life is declared. The environmental impact due to the use phase is null.
DESCRIPTION OF THE SYSTEM BOUNDARY (X = INCLUDED IN LCA; MND = MODULE OR INDICATOR NOT DECLARED; MNR
= MODULE NOT RELEVANT)
Benefits and
Construction loads beyond
Product stage Use stage End of life stage
process stage the system
boundaries
la ire ta m w a Ry lp p u s tro p s n a rT g n iru tc a fu n a M e h t m o rf tro p s n a rTe tis e h t o t e ta g y lb m e s s A e s U e c n a n e tn ia M ria p e R tn e m e c a lp e R tn e m h s ib ru fe R y g re n e la n o ita re p Oe s u re ta w la n o ita re p Oe s u n o itc u rts n o c -e Dn o itilo m e d tro p s n a rT g n is s e c o rp e ts a W la s o p s iD -e s u e R-y re v o c e R-g n ilc y c e Rla itn e to p
A1 A2 A3 A4 A5 B1 B2 B3 B4 B5 B6 B7 C1 C2 C3 C4 D
X X X MND X MND MND MNR MNR MNR MND MND X X X X X
RESULTS OF THE LCA - ENVIRONMENTAL IMPACT according to EN 15804+A2: 1 Kg Average PregyMetal - Z100 galvanized
steel profiles 1mm thickness
Parameter Unit A1 A2 A3 A5 C1 C2 C3 C4 D
GWP-total kg CO 2 eq 2.17E+00 3.88E-02 3.31E-03 7.7E-03 5.71E-03 1.92E-02 1.73E-02 6.35E-04 -1.2E+00
GWP-fossil kg CO 2 eq 2.17E+00 3.87E-02 3.29E-03 7.21E-03 5.23E-03 1.92E-02 1.73E-02 6.34E-04 -1.19E+00
GWP-biogenic kg CO 2 eq -8.97E-04 3.72E-05 2.23E-05 5.03E-04 4.79E-04 1.84E-05 1.66E-05 4.1E-07 -2.43E-03
GWP-luluc kg CO 2 eq 1.75E-03 1.86E-05 2.04E-06 1.7E-06 8.05E-07 9.21E-06 8.29E-06 3.73E-07 -5.12E-04
ODP kg CFC11 eq 4.72E-08 8.26E-10 1.59E-10 1.56E-10 1.14E-10 4.09E-10 3.68E-10 1.76E-11 -2.19E-08
AP mol H+ eq 2.15E-02 1.56E-04 1.36E-05 2.6E-05 1.84E-05 7.74E-05 6.97E-05 4.58E-06 -4.86E-03
EP-freshwater kg P eq 1E-03 2.66E-06 6.86E-07 9.42E-07 8.08E-07 1.32E-06 1.19E-06 5.06E-08 -5.55E-04
EP-marine kg N eq 2.51E-03 5.96E-05 2.67E-06 6.01E-06 3.14E-06 2.95E-05 2.66E-05 1.76E-06 -1.08E-03
EP-terrestrial mol N eq 7.8E-02 6.36E-04 2.58E-05 6.63E-05 3.56E-05 3.15E-04 2.84E-04 1.88E-05 -1.15E-02
kg NMVOC
POCP 1.03E-02 2.29E-04 5.18E-05 2.64E-05 1.53E-05 1.13E-04 1.02E-04 6.56E-06 -5.46E-03
eq
ADPE kg Sb eq 2.33E+01 5.39E-01 1.1E-01 1.07E-01 8E-02 2.67E-01 2.4E-01 1.51E-02 -1.19E+01
ADPF MJ 4.17E-05 1.22E-07 2.29E-08 1.52E-08 9.04E-09 6.04E-08 5.44E-08 8.44E-10 -9.83E-06
m3 world eq
WDP 6.48E-01 2.23E-03 6.68E-04 3.31E-03 3.21E-03 1.1E-03 9.92E-04 6.7E-04 -2.45E-01
deprived
GWP = Global warming potential; ODP = Depletion potential of the stratospheric ozone layer; AP = Acidification potential of land and water; EP =
Eutrophication potential; POCP = Formation potential of tropospheric ozone photochemical oxidants; ADPE = Abiotic depletion potential for non-fossil
resources; ADPF = Abiotic depletion potential for fossil resources; WDP = Water (user) deprivation potential)
RESULTS OF THE LCA - INDICATORS TO DESCRIBE RESOURCE USE according to EN 15804+A2: 1 Kg Average PregyMetal -
Z100 galvanized steel profiles 1mm thickness
Parameter Unit A1 A2 A3 A5 C1 C2 C3 C4 D
PERE MJ 1.8E+00 8.36E-03 2.58E-03 2.07E-02 2.02E-02 4.14E-03 3.73E-03 1.28E-04 0
PERM MJ 0 0 0 0 0 0 0 0 0
PERT MJ 1.8E+00 8.36E-03 2.58E-03 2.07E-02 2.02E-02 4.14E-03 3.73E-03 1.28E-04 0
PENRE MJ 2.47E+01 5.73E-01 1.17E-01 1.16E-01 8.65E-02 2.84E-01 2.55E-01 1.61E-02 0
PENRM MJ 0 0 0 0 0 0 0 0 0
PENRT MJ 2.47E+01 5.73E-01 1.17E-01 1.16E-01 8.65E-02 2.84E-01 2.55E-01 1.61E-02 0
SM kg 3.5E-01 0 0 0 0 0 0 0 0
RSF MJ 0 0 0 0 0 0 0 0 0
NRSF MJ 0 0 0 0 0 0 0 0 0
FW m3 1.96E-02 7.68E-05 2.22E-05 9.02E-05 8.63E-05 3.8E-05 3.42E-05 1.61E-05 -6.69E-03
PERE = Use of renewable primary energy excluding renewable primary energy resources used as raw materials; PERM = Use of renewable primary
energy resources used as raw materials; PERT = Total use of renewable primary energy resources; PENRE = Use of non-renewable primary energy
excluding non-renewable primary energy resources used as raw materials; PENRM = Use of non-renewable primary energy resources used as raw
materials; PENRT = Total use of non-renewable primary energy resources; SM = Use of secondary material; RSF = Use of renewable secondary fuels;
NRSF = Use of non-renewable secondary fuels; FW = Use of net fresh water
RESULTS OF THE LCA – WASTE CATEGORIES AND OUTPUT FLOWS according to EN 15804+A2:
1 Kg Average PregyMetal - Z100 galvanized steel profiles 1mm thickness
Parameter Unit A1 A2 A3 A5 C1 C2 C3 C4 D
HWD kg 3.99E-04 3.43E-06 5.7E-07 4.43E-07 2.69E-07 1.7E-06 1.53E-06 8.02E-08 -1.01E-04
NHWD kg 5.01E-01 2.63E-02 3.57E-04 1.36E-03 2.38E-04 1.3E-02 1.17E-02 1E-01 -4.95E-01
RWD kg 3.04E-05 1.75E-07 6.8E-08 1.84E-07 1.73E-07 8.67E-08 7.8E-08 2.24E-09 -1.05E-05
CRU kg 0 0 0 0 0 0 0 0 0
MFR kg 0 0 9.5E-03 5E-02 0 0 9E-01 0 0
5 Environmental Product Declaration - Etex Building Performance SpA - PregyMetal - Z100 galvanized steel profiles 1mm thickness
MER kg 0 0 0 0 0 0 0 0 0
EEE MJ 0 0 0 0 0 0 0 0 0
EET MJ 0 0 0 0 0 0 0 0 0
HWD = Hazardous waste disposed; NHWD = Non-hazardous waste disposed; RWD = Radioactive waste disposed; CRU = Components for re-use;
MFR = Materials for recycling; MER = Materials for energy recovery; EEE = Exported electrical energy; EET = Exported thermal energy
RESULTS OF THE LCA – additional impact categories according to EN 15804+A2-optional:
1 Kg Average PregyMetal - Z100 galvanized steel profiles 1mm thickness
Parameter Unit A1 A2 A3 A5 C1 C2 C3 C4 D
Disease
PM 2.73E-07 3.09E-09 1.36E-10 2.23E-10 8.72E-11 1.53E-09 1.38E-09 1E-10 -8.72E-08
incidence
IR kBq U235 eq 1.21E-01 7.21E-04 2.71E-04 7.04E-04 6.6E-04 3.57E-04 3.21E-04 9.59E-06 -4.16E-02
ETP-fw CTUe 2.08E+01 2.85E-01 4.29E-02 2.44E-02 9.74E-03 1.41E-01 1.27E-01 7.43E-03 -2.96E+00
HTP-c CTUh 5.62E-08 4.99E-10 5.34E-11 5.62E-11 3.23E-11 2.47E-10 2.22E-10 7.34E-12 -2.86E-08
HTP-nc CTUh 1.46E-08 1.72E-11 2.67E-12 2.17E-12 1.36E-12 8.54E-12 7.69E-12 2.59E-13 -7.25E-09
SQP SQP 7.4E+00 3.2E-01 1.1E-02 2.63E-02 1.23E-02 1.59E-01 1.43E-01 3.01E-02 -3.81E+00
PM = Potential incidence of disease due to PM emissions; IR = Potential Human exposure efficiency relative to U235; ETP-fw = Potential comparative
Toxic Unit for ecosystems; HTP-c = Potential comparative Toxic Unit for humans (cancerogenic); HTP-nc = Potential comparative Toxic Unit for humans
(not cancerogenic); SQP = Potential soil quality index
Disclaimer 1 – for the indicator “Potential Human exposure efficiency relative to U235”. This impact category deals mainly with the
eventual impact of low-dose ionizing radiation on human health of the nuclear fuel cycle. It does not consider effects due to possible
nuclear accidents, occupational exposure or radioactive waste disposal in underground facilities. Potential ionizing radiation from the
soil, radon and from some construction materials is also not measured by this indicator.
Disclaimer 2 – for the indicators “abiotic depletion potential for non-fossil resources”, “abiotic depletion potential for fossil resources”,
“water (user) deprivation potential, deprivation-weighted water consumption”, “potential comparative toxic unit for ecosystems”,
“potential comparative toxic unit for humans – cancerogenic”, “Potential comparative toxic unit for humans - not cancerogenic”,
“potential soil quality index”. The results of this environmental impact indicator shall be used with care as the uncertainties on these
results are high as there is limited experience with the indicator.
6. LCA: Interpretation
Product stage (modules A1-A3) is responsible for the biggest impacts on the Global Warming Potential is due to its
share of the impact for most indicators. About 90% of the production, especially in the raw materials phase in A1.
7. Requisite evidence
The products covered by this document comply with EN 14195 type of surface treatment.
regarding their field of application and with EN 10346 for the
8. References
Standards: UNI ISO 45001:2018 - Occupational health and safety
management systems
EN 15804EN15804:2012+A1 2013, Sustainability of
construction works— Environmental Product Declarations — UNI EN ISO 14001:2015 - Environmental management
Core rules for theproduct category of construction products.EN systems
15804.
ISO 15686 - Buildings and constructed assets
EN 15804:2012+A2:2019+AC:2021, Sustainability
ofconstruction works — Environmental Product Declarations —
Core rules for the product category of construction ISO 13501:1 - Petroleum and natural gas industries
products.ISO 14025.
European Regulation EC/1272/2008 -Regulation (EC) No
EN ISO 14025:2011, Environmental labels and declarations — 1272/2008 of the European Parliament and of the Council of 16
Type III environmental declarations — Principles December 2008 on classification, labelling and packaging of
andprocedures. substances and mixtures, amending and repealing Directives
67/548/EEC and 1999/45/EC, and amending Regulation (EC)
No 1907/2006 (Text with EEA relevance)
EN 14195:2005 - Metal framing components for gypsum board
systems - Definitions, requirements and test methods and the
CE-marking. EN 14195 - Metal framing components for gypsum board
systems
UNI EN ISO 9001:2015 - Quality management systems
EN 10346 - Continuously hot-dip coated steel flat products
6 Environmental Product Declaration - Etex Building Performance SpA - PregyMetal - Z100 galvanized steel profiles 1mm thickness
Further References: Candidate List of Substances of Very High Concern for
Authorisation' (SVHC).
IBU 2021
Institut Bauen und Umwelt e.V.: General Instructions for EWC-Stat categories - European Waste Classification.
theEPD programme of Institut Bauen und Umwelt e.V.,
Version2.0, Berlin: Institut Bauen und Umwelt e.V.,
2021www.ibu-epd.com. Federal office for building and regional planning (BBSR) BNB
" (http://www.nachhaltigesbauen.de/baustoff-und-
gebaeudedaten/nutzungsdauern-von-bauteilen.html).
PCR Part A - Calculation Rules for the Life Cycle As-sessment
and Requirements on the Project Re-port according to EN
15804+A2:2019. Version 6, 12/07/2023 Title of the software/database:
PCR Part B - Requiment on the EPD for Structural steel, V.1, Software: SimaPro 9.5.0.1
06/04/2023. Database: Ecoinvent 3.9.1
Regulation (EU) No. 305/2011 -Regulation (EU) No 305/2011 of The literature referred to in the Environmental Product
the European Parliament and of the Council of 9 March 2011 Declaration must be listed in full.Standards already fully quoted
laying down harmonised conditions for the marketing of in the EPD do not need to be listed here again.
construction products and repealing Council Directive The current version of PCR Part A and PCR Part B of the PCR
89/106/EEC Text with EEA relevance document on which they are based must be referenced.
7 Environmental Product Declaration - Etex Building Performance SpA - PregyMetal - Z100 galvanized steel profiles 1mm thickness
Publisher
Institut Bauen und Umwelt e.V. +49 (0)30 3087748- 0
Hegelplatz 1 info@ibu-epd.com
10117 Berlin www.ibu-epd.com
Germany
Programme holder
Institut Bauen und Umwelt e.V. +49 (0)30 3087748- 0
Hegelplatz 1 info@ibu-epd.com
10117 Berlin www.ibu-epd.com
Germany
Author of the Life Cycle Assessment
Greenwich srl +390354948794
Via Presolana 2/4 info@greenwichsrl.it
24030 Medolago https://greenwichsrl.it/
Italy
Owner of the Declaration
Etex Building Performance International +32 2 778 12 11
Rue Marcel Demonque 500 info@etexgroup.com
84915 Avignon Cedex 9 www.etexgroup.com
France
8 Environmental Product Declaration - Etex Building Performance SpA - PregyMetal - Z100 galvanized steel profiles 1mm thickness
