ENVIRONMENTAL PRODUCT DECLARATION
as per ISO 14025 and EN 15804+A2
Owner of the Declaration voestalpine AG
Publisher Institut Bauen und Umwelt e.V. (IBU)
Programme holder Institut Bauen und Umwelt e.V. (IBU)
Declaration number EPD-VOE-20230107-IBC2-EN
Issue date 09.05.2023
Valid to 08.05.2028
Shaped Wire
voestalpine Wire Austria GmbH
www.ibu-epd.com | https://epd-online.com
1. General Information
voestalpine Wire Austria GmbH Shaped Wire
Programme holder Owner of the declaration
IBU – Institut Bauen und Umwelt e.V. voestalpine AG
Hegelplatz 1 voestalpine-Straße 3
10117 Berlin 4020 Linz
Germany Austria
Declaration number Declared product / declared unit
EPD-VOE-20230107-IBC2-EN 1 tonne of shaped wire
This declaration is based on the product category rules: Scope:
Structural steels, 01.08.2021 This EPD is based on a declared unit of 1 metric tonne of average
(PCR checked and approved by the SVR) voestalpine shaped wire produced at the production site in Bruck a.d. Mur
(Austria).
The owner of the declaration shall be liable for the underlying information
Issue date and evidence; the IBU shall not be liable with respect to manufacturer
information, life cycle assessment data and evidences.
09.05.2023
The EPD was created according to the specifications of EN 15804+A2. In
the following, the standard will be simplified as EN 15804.
Valid to
08.05.2028 Verification
The standard EN 15804 serves as the core PCR
Independent verification of the declaration and data according to ISO
14025:2011
internally X externally
Dipl.-Ing. Hans Peters
(Chairman of Institut Bauen und Umwelt e.V.)
Florian Pronold Prof. Dr. Birgit Grahl,
(Managing Director Institut Bauen und Umwelt e.V.) (Independent verifier)
1 Environmental Product Declaration - voestalpine Wire Austria GmbH - Shaped Wire
2. Product
2.1 Product description/Product definition
Shaped wires are used to produce parts for a wide field of
different applications, such as in automotive industry, oil & gas,
energy, agriculture, food industry, machine building,
transportation, and much more. By using drawing and cold
rolling voestalpine Wire Austria can produce the easiest and
most complex geometries in combination with modelling and
simulation of the cold rolling steps needed. voestalpine Wire
Austria has a big knowledge on how to process the round wire
rod to the final needed shape and needed material
characteristics of the customers. Various steel grades are processed at the rolling facility of
voestalpine Wire Austria GmbH.
In order to fulfill certain requirements concerning mechanical
properties and deformability, specific chemical compositions, as Carbon steel grades:
well as optimized production processes are used to produce Low alloyed carbon steel (carbon content up to max. 1,05 %)
the wires.
To ensure high-quality standards, all products are Spring steel grades:
manufactured under optimized process conditions, such as: Steels according to ISO 10270-1 and EN 10089 are used to
produce shaped spring steel wire. The following alloys are
• High degree of purity
suitable to produce quenched and tempered springs and are a
• Low core segregation
selection from the voestalpine Wire Austria GmbH product
• Optimized annealing conditions
range but only in soft execution – quenching is not in the
• Continuous quality inspections and several special
production range.
testing options
• End-to-end traceability of all production and test
parameters
• Greatest possible flexibility as the result of an integrated
production chain
• Strict adherence to schedules, and partnerships with our
customers
• Technical and sales service
For the use and application of the product the respective
national provisions at the place of use apply, in Germany for
Customer-specific changes to the alloy composition can occur
example the building codes of the federal states and the
on request.
corresponding national specifications.
2.2 Application High alloy special steel grades:
Shaped wire products from voestalpine Wire Austria GmbH are Special grades upon request.
used to produce a variety of components ranging from safety
parts, fasteners, fixations, chains and armoring wires. Performance data of the product with respect to its
characteristics in accordance with the relevant technical
Carbon steel shaped wires are optimized to produce armor wire provision (no CE-marking).
for flexile pipes, ropes, retaining rings, springs and automotive
2.4 Delivery status
parts.
By applying the EN 10278 standard, tightest width and height
tolerances are guaranteed for all types of wire products.
Spring steel shaped wire products from voestalpine Wire
Shaped wires produced have following production range.
Austria GmbH are characterized by a high yield strength to
tensile strength ratio and are therefore well suited to produce a
wide variety of spring elements.
2.3 Technical Data
This EPD applies to all shaped wires from voestalpine Wire
Austria GmbH, which is why a general statement about
mechanical parameters is not possible. The technical data
given for the products are generic literature data for steel as
described e.g. in Key to Steel. No product specific test rules are
applicable to the data given:
Constructional data
In terms of surface finish, a distinction is made between:
• phosphate-free
• phosphate coated, with a soap or lime coating
2 Environmental Product Declaration - voestalpine Wire Austria GmbH - Shaped Wire
• bright drawn
• oiled inline
• oil dipped for final annealed shaped wire
All produced wires are supplied in coils with different coil types:
• catch weight coils
• coreless coils
• steel or wooden reels
The outer diameter and weight of the coils vary between 400 to
1350 mm and 250 to 3000 kg, depending on the wire size.
2.5 Base materials/Ancillary materials
Base materials:
The starting product for shaping wires is hot-rolled wire, which
is produced at the voestalpine Wire Rod Austria site. The basic
material for this is in turn crude steel, which consists of about
85 % pig iron and about 15 % scrap and alloying elements.
This product/article/at least one partial article contains
substances listed in the candidate list (date: 16.1.2020)
exceeding 0.1 percentage by mass: no.
This product/article/at least one partial article contains other
carcinogenic, mutagenic, reprotoxic (CMR) substances in The annealing of the coils takes place in a bell-type annealing
categories 1A or 1B which are not on the candidate list, furnace at temperatures and times of around 700 °C and 12
exceeding 0.1 percentage by mass: no. hours, or at specially developed temperature/time curves.
Biocide products were added to this wire product, or it has been 2.7 Environment and health during manufacturing
treated with biocide products (this then concerns a treated The voestalpine Wire Austria site is certified according to EMAS
product as defined by the (EU) Ordinance on Biocide Products III, ISO 9001, ISO 50001 and ISO 14001. As part of the
No. 528/2012): no. environmental declarations required by EMAS, voestalpine
continuously publishes environmentally relevant data and facts
2.6 Manufacture
about the site.
The starting material to produce shaped wires is low alloyed
steel, which is mainly produced at voestalpine Stahl Donawitz At the Bruck/Mur site, investments are constantly being made in
GmbH via the primary route (blast furnace, LD steel mill, ladle the expansion of environmental protection measures in order to
furnace). The steel is cast into blooms using a continuous be able to reduce emissions to air and water to a minimum.
casting process.
All operating facilities that have been approved in accordance
In a further step, the blooms are rolled to the desired dimension with the environmental impact assessment procedure are also
in the wire rod rolling mill of voestalpine Wire Rod Austria periodically inspected by the authorities as part of
GmbH. The diameters of the rolled wire rod vary between 5 and environmental inspections.
31 mm. After the rolling process, the wires are delivered by train
to voestalpine Wire Austria GmbH in Bruck an der Mur. 2.8 Product processing/Installation
Shaped wire products from voestalpine Wire Austria GmbH are
In a first step, the wire rods are pickled in hydrochloric acid. At processed by a broad range of different customers in the
the drawing and rolling facility of voestalpine Wire Austria respective factories. Depending on the desired wire
GmbH the wires are further processed according to EN 10263 specification, the wire is further processed in different ways,
specifications. e.g. cold heading, turning or spring coiling.
2.9 Packaging
The declared product is delivered on wooden pallets. Pallets
treated according to the ISPM 15 standard are used on
customer request. The packaging of the drawn wires varies
according to customer requirements, therefore various
packaging materials are used to protect the wires from
environmental influences, e.g.:
• PE (polyethylene) stretch foil
• LDPE (low-densitiy polyethylene) foil
• VCI (colative chemical inhibitors) foil
• crepe paper
• cardboard boxes
• wooden boxes
2.10 Condition of use
There is no change in material composition over the service life
of the product. If used as intended, no effects on the
environment are to be expected.
3 Environmental Product Declaration - voestalpine Wire Austria GmbH - Shaped Wire
Mechanical destruction
2.11 Environment and health during use Unpredictable mechanical impact on the declared products has
During the use of steel wire products, no effects on human and no negative consequences on the environment due to the
animal health and no harmful emissions to air, soil and water plastic deformability of steel.
are expected.
2.14 Re-use phase
2.12 Reference service life Wire from voestalpine can either be reused or recycled and
Due to the variety of applications and their stresses, reintroduced into the steel industry as a secondary raw material
voestalpine Wire Austria GmbH does not specify a reference via recycling companies.
service life for their wire products. Corrosive atmospheres must
be avoided to guarantee a full lifetime of functionality. 2.15 Disposal
The declared product can be fully used as a recycling raw
2.13 Extraordinary effects material. The waste code according to the European Waste
Fire Catalogue is: 17 04 05 (iron and steel). The waste type is
Steel wires are not flammable, therefore no flammable gases or equivalent to the key number 35103 according to the nationally
vapours escape. applicable Waste Catalogue by-law.
Water 2.16 Further information
No negative consequences for the environment are to be Further information on the product is available on the website at
expected under the influence of water. https://www.voestalpine.com/wiretechnology/en/drawn-wire/flat-
and-shaped-wire-/
3. LCA: Calculation rules
Module C2 | Transport
3.1 Declared Unit The transport to the disposal of the material is estimated
This environmental product declaration refers to a declared unit declaring a 50 km radius to the waste processing.
of 1 tonne of average shaped wire.
Declared unit Module C3 | Waste processing
Product flows that reach Module D for recycling leave the
Name Value Unit
product system in C3. Environmental impacts resulting from the
Declared unit 1 t
grinding and sorting of steel scrap are not included due to the
Density 7850 kg/m3 negligible expected environmental impact.
For the calculation of the declared average, input and
Module C4 | Landfilling
production quantities for the entire calendar year 2018 were
Module C4 declares the environmental impacts incurred by
taken into account and broken down to the declared product
landfilling (5 % of the product).
group. The calculated results can thus be considered
representative for the declared product portfolio of shaped wire
Module D | Benefits and loads beyond the system
of voestalpine Wire Austria GmbH.
boundary
The potential for substituting primary steel with a recycling
A linear correlation of the environmental impacts with the
scenario (95 % of the product) is outlined in Module D.
product weight is to be expected. Therefore, the conversion
from the declared unit to a specific product is possible using a
3.3 Estimates and assumptions
mass-specific scaling factor.
All assumptions are verified through detailed documentation
3.2 System boundary and correspond to the best possible representation of reality
based on the available data. Regional applicability of the used
The life cycle assessment of average shaped wire refers to a
background data refers to average data under European or
cradle-to-gate analysis with modules (A1–A3 + C +D).
German conditions taken from the GaBi-database. German
Subsequent life cycle phases are part of the analysis:
data were used for the Austrian market whenever European or
Austrian average data were not available.
Module A1–A3 | Production stage
The production stage includes the burdens of the production of
3.4 Cut-off criteria
shaped wire of voestalpine Wire Austria GmbH at the
All inputs and outputs for which data are available are included
production site in Bruck a.d. Mur. Most of the used steel wire is
in the LCA model. Data gaps are filled with conservative
provided by the voestalpine Wire Rod Austria from St. Peter
assumptions from average data (when available) or with
Freienstein. Thus, the upstream environmental impact of the
generic data and are documented accordingly. Only data with a
steel supplied is represented by primary data of the respective
contribution of less than 1 % were cut off. Ignoring such data is
production site. Material and energy flows for the pickling,
justified based on the irrelevance of the expected effect.
drawing, cold rolling, annealing and patenting are considered.
Processes, materials, or emissions known to make a significant
Electricity at Bruck a. d. Mur is provided from 100 % renewable
contribution to the environmental effects of the products under
energy (emission factor GWP-total: 14 g CO equivalents/kWh).
2- examination have not been neglected. All relevant data were
Thermal energy provision is based on natural gas. Module A1– collected comprehensively. It is assumed that the data have
A3 also includes the production of the packaging. been completely recorded and the overall total of ignored input
flows do not amount to more than 5 % of total energy and mass
Module C1 | Deconstruction and demolition flows.
It is assumed that the product is not connected with other
materials and can therefore be dismantled. Associated efforts Environmental impacts of machines, plant and infrastructure
are negligible, no environmental impacts from the were not included.
deconstruction of the products are declared.
3.5 Background data
4 Environmental Product Declaration - voestalpine Wire Austria GmbH - Shaped Wire
This study uses generic background data for the evaluation of
upstream environmental impacts from GaBi-database 2021.1 3.9 Allocation
and is modelled in GaBi-software version 10. The primary data for the upstream production of the steel billets
were allocated using the partitioning approach developed by
3.6 Data quality worldsteel 2014 for calculating life cycle inventories of co-
The foreground data collected at voestalpine Wire Austria products in steel production, which is in line with the provisions
GmbH are based on the quantities used and volumes produced of EN 15804. The so-called partitioning approach provides for
annually. Process data were collected by voestalpine in the the allocation of environmental effects on the steelmaking
course of reporting to official agencies. Data on material and process and the emerging byproducts based on physical
energy use originate from material-specific throughput relations. Material-inherent flow properties are, thus, taken into
measurements of various processes as well as from controlling. account.
The technological, geographical and time-related
representativeness of the data base was kept in mind when Economic allocation is not considered as referring byproducts
selecting background data. Whenever specific data were and co-products are notdirectly tradable goods. Furthermore,
missing, either generic datasets or representative average data long-term contracts for the sale of thebyproducts exist, and the
were used instead. The implemented GaBi background negotiated prices are, therefore, not subject to market
datasets are not more than ten years old. dynamics.
3.7 Period under review 3.10 Comparability
Foreground data were collected in the 2018 production year, Basically, a comparison or an evaluation of EPD data is only
and the data are based on the volumes produced on an annual possible if all the data sets to be compared were created
basis. according to EN 15804 and the building context, respectively
the product-specific characteristics of performance, are taken
3.8 Geographic Representativeness into account. The GaBi background database was used to
Land or region, in which the declared product system is calculate the LCA (GaBi 10; 2021.1).
manufactured, used or handled at the end of the product´s
lifespan: Austria
4. LCA: Scenarios and additional technical information
The end-of-life scenario used in this LCA study is based on the
Characteristic product properties of biogenic carbon following assumptions and thus complies with the specifications
The declared product does not contain any biogenic carbon. published in ökobaudat 2022:
Information on describing the biogenic Carbon Content at End of life (C1–C4)
factory gate
Name Value Unit
Name ValueUnit
Collected separately (steel) 1000 kg
Biogenic carbon content in accompanying kg
6.28 Recycling 95 % 950 kg
packaging C
Landfilling 5 % 50 kg
The carbon stored in the packaging was taken into account as
"CO -neutral". Thus the storage effect of the carbon bound in Reuse, recovery and/or recycling potentials (D), relevant
2
scenario information
the packaging is not included in the calculation but is
considered as emitted immediately. Name Value Unit
Net flow of steel scrap 918 kg
This scenario contains a recycling rate of 95 %. Since
voestalpine externally purchases scrap for steel production, this
is offset against the steel scrap for recycling (net flow).
Installation into the building (A5)
The end-of-life of the packaging materials is not declared in
Module A5.
Name Value Unit
Packaging (binding wire, packaging strips) 0.66 kg
Packaging (plastic) 0.33 kg
Packaging (cardboard) 0.075 kg
Packaging (wood) 14 kg
5 Environmental Product Declaration - voestalpine Wire Austria GmbH - Shaped Wire
5. LCA: Results
The following table contains the LCA results for a declared unit of 1 tonne of shaped wire.
DESCRIPTION OF THE SYSTEM BOUNDARY (X = INCLUDED IN LCA; ND = MODULE OR INDICATOR NOT DECLARED; MNR =
MODULE NOT RELEVANT)
Benefits and
Construction loads beyond
Product stage Use stage End of life stage
process stage the system
boundaries
la ire ta m w a Ry lp p u s tro p s n a rT g n iru tc a fu n a M e h t m o rf tro p s n a rTe tis e h t o t e ta g y lb m e s s A e s U e c n a n e tn ia M ria p e R tn e m e c a lp e R tn e m h s ib ru fe R y g re n e la n o ita re p Oe s u re ta w la n o ita re p Oe s u n o itc u rts n o c -e Dn o itilo m e d tro p s n a rT g n is s e c o rp e ts a W la s o p s iD -e s u e R-y re v o c e R-g n ilc y c e Rla itn e to p
A1 A2 A3 A4 A5 B1 B2 B3 B4 B5 B6 B7 C1 C2 C3 C4 D
X X X MND MND MND MND MNR MNR MNR MND MND X X X X X
RESULTS OF THE LCA - ENVIRONMENTAL IMPACT according to EN 15804+A2: 1 tonne shaped wire
Parameter Unit A1-A3 C1 C2 C3 C4 D
Global Warming Potential total (GWP-total) kg CO 2 eq 3.08E+03 0 3.02E+00 0 2.42E+00 -1.56E+03
Global Warming Potential fossil fuels (GWP-fossil) kg CO 2 eq 3.07E+03 0 3E+00 0 2.44E+00 -1.56E+03
Global Warming Potential biogenic (GWP-biogenic) kg CO 2 eq 1.78E+01 0 -3.56E-03 0 -2.5E-02 -1.01E+00
Global Warming Potential luluc (GWP-luluc) kg CO 2 eq 1.1E+00 0 2.44E-02 0 2.44E-03 2.25E-01
Depletion potential of the stratospheric ozone layer (ODP) kg CFC11 eq 9.41E-11 0 5.9E-16 0 5.77E-15 -2.6E-12
Acidification potential of land and water (AP) mol H+ eq 9.59E+00 0 9.92E-03 0 7.78E-03 -2.8E+00
Eutrophication potential aquatic freshwater (EP-freshwater) kg P eq 1.61E-02 0 8.88E-06 0 1.86E-06 -3.18E-04
Eutrophication potential aquatic marine (EP-marine) kg N eq 2.31E+00 0 4.55E-03 0 1.93E-03 -4.17E-01
Eutrophication potential terrestrial (EP-terrestrial) mol N eq 2.46E+01 0 5.08E-02 0 2.12E-02 -4.06E+00
Formation potential of tropospheric ozone photochemical oxidants kg NMVOC
7.72E+00 0 8.94E-03 0 6.08E-03 -2.13E+00
(POCP) eq
Abiotic depletion potential for non fossil resources (ADPE) kg Sb eq 5.29E-03 0 2.65E-07 0 1.68E-07 -3.39E-03
Abiotic depletion potential for fossil resources (ADPF) MJ 2.8E+04 0 3.98E+01 0 3.56E+01 -1.36E+04
m3 world eq
Water use (WDP) 6.05E+02 0 2.77E-02 0 -2.89E-02 -3.06E+02
deprived
RESULTS OF THE LCA - INDICATORS TO DESCRIBE RESOURCE USE according to EN 15804+A2: 1 tonne shaped wire
Parameter Unit A1-A3 C1 C2 C3 C4 D
Renewable primary energy as energy carrier (PERE) MJ 2.89E+03 0 2.29E+00 0 2.57E+00 1.25E+03
Renewable primary energy resources as material utilization
MJ 2.32E+02 0 0 0 0 0
(PERM)
Total use of renewable primary energy resources (PERT) MJ 3.12E+03 0 2.29E+00 0 2.57E+00 1.25E+03
Non renewable primary energy as energy carrier (PENRE) MJ 2.81E+04 0 4E+01 0 3.56E+01 -1.36E+04
Non renewable primary energy as material utilization (PENRM) MJ 1.46E+01 0 0 0 0 0
Total use of non renewable primary energy resources (PENRT) MJ 2.81E+04 0 4E+01 0 3.56E+01 -1.36E+04
Use of secondary material (SM) kg 1.24E+02 0 0 0 0 9.18E+02
Use of renewable secondary fuels (RSF) MJ 0 0 0 0 0 0
Use of non renewable secondary fuels (NRSF) MJ 0 0 0 0 0 0
Use of net fresh water (FW) m3 1.8E+01 0 2.62E-03 0 3.67E-04 -6.86E+00
RESULTS OF THE LCA – WASTE CATEGORIES AND OUTPUT FLOWS according to EN 15804+A2:
1 tonne shaped wire
Parameter Unit A1-A3 C1 C2 C3 C4 D
Hazardous waste disposed (HWD) kg 2.25E-03 0 2.11E-09 0 6.3E-09 3.78E-06
Non hazardous waste disposed (NHWD) kg 7E+01 0 6.27E-03 0 5.01E+01 1.63E+02
Radioactive waste disposed (RWD) kg 1.33E-01 0 7.25E-05 0 4.05E-04 4.91E-04
Components for re-use (CRU) kg 0 0 0 0 0 0
Materials for recycling (MFR) kg 0 0 0 9.5E+02 0 0
Materials for energy recovery (MER) kg 0 0 0 0 0 0
Exported electrical energy (EEE) MJ 0 0 0 0 0 0
Exported thermal energy (EET) MJ 0 0 0 0 0 0
RESULTS OF THE LCA – additional impact categories according to EN 15804+A2-optional:
1 tonne shaped wire
Parameter Unit A1-A3 C1 C2 C3 C4 D
Disease
Incidence of disease due to PM emissions (PM) ND ND ND ND ND ND
incidence
Human exposure efficiency relative to U235 (IR) kBq U235 eq ND ND ND ND ND ND
Comparative toxic unit for ecosystems (ETP-fw) CTUe ND ND ND ND ND ND
Comparative toxic unit for humans (carcinogenic) (HTP-c) CTUh ND ND ND ND ND ND
6 Environmental Product Declaration - voestalpine Wire Austria GmbH - Shaped Wire
Comparative toxic unit for humans (noncarcinogenic) (HTP-nc) CTUh ND ND ND ND ND ND
Soil quality index (SQP) SQP ND ND ND ND ND ND
The additional and optional impact categories according to EN 15804+A2 are not declared, as the uncertainty of these indicators is to
be classified as high.
Disclaimer 1 – for the indicator potential human exposure efficiency relative to U235:
This impact category deals mainly with the eventual impact of low dose ionizing radiation on human health of the nuclear fuel cycle. It
does not consider effects due to possible nuclear accidents, occupational exposure nor radioactive waste disposal in underground
facilities. Potential ionizing radiation from the soil, from radon and from some construction materials is also not measured by this
indicator.
Disclaimer 2 – for the indicators abiotic depletion potential for non-fossil resources, abiotic depletion potential for fossil resources, water
(user) deprivation potential, deprivation weighted water consumption, eutrophication fraction of nutrients reaching freshwater end
compartment, potential comparative toxic unit for humans cancerogenic, potential comparative toxic unit for humans not cancerogenic,
potential soil quality index:
The results of this environmental impact indicator shall be used with care as the uncertainties on these results are high or as there is
limited experience with the indicator.
6. LCA: Interpretation
The following interpretation contains a summary of the LCA
results referenced to a declared unit of 1 tonne of shaped wire.
A comparison of the individual lifecycle phases results in a clear
dominance of the production phase (modules A1–A3). The Most of the potential environmental impacts of the production
environmental effects in the production phase are mainly phase (module A1–A3) of the shaped wire can be traced back
dominated by the direct process emissions of billet production. to the upstream supply of the wire rod. The production of
shaped wire at the production site at Bruck contributes app. 5
As a result of product recyclability, the material removed at the % to global warming potential.
end of life can substitute primary steel. According to the set
method, the first step is to saturate the secondary material used A linear correlation of the environmental impacts with the
in module A with material from module C. The excess amount product weight is to be expected. Therefore, the conversion
from module C ('net flow') can substitute primary steel and from the declared unit to a specific product is possible using a
leads to corresponding substitution potentials in module D. mass-specific scaling factor.
The environmental impact of the transport of the products to All primary data were specifically broken down to the declared
recycling (C2) as well as landfilling of the losses at the end of product group. As a result, the representativity of the results for
life (C4) represents a minor contribution to the overall the declared product group is to be expected as high.
environmental impact of the product.
7. Requisite evidence
7 Environmental Product Declaration - voestalpine Wire Austria GmbH - Shaped Wire
Not relevant for this EPD.
8. References
Standards Chemicals Agency.
EN 10027-2 EMAS III
DIN EN 10027-2:2015-07, Designation systems for steels - Part Regulation (EC) No 1221/2009 of the European parliament and
2: Numerical system. of the council of 25 November 2009 on the voluntary
participation by organisations in a Community eco-management
EN 10089 and audit scheme (EMAS), repealing Regulation (EC) No
DIN EN 10089-2:2003-04, Hot rolled steels for quenched and 761/2001 and Commission Decisions 2001/681/EC and
tempered springs - Technical delivery conditions. 2006/193/EC.
EN 10263 European Waste Catalogue
DIN EN 10263-1:2018-02, Steel rod, bars and wire for cold Guidance on classification of waste according to EWC Stat
heading and cold extrusion - Part 1: General technical delivery categories. Supplement to the Manual for the Implementation of
conditions. the Regulation (EC) No 2150/2002 on Waste Statistics.
Commission of the European Communities, EUROSTAT.
EN 10278
DIN EN 10278:1999-12, Dimensions and tolerances of bright GaBi
steel products. GaBi 10, Software System and Database for Life Cycle
Engineering. DB 2021.1. Sphera, 1992-2021. Available in:
EN 15804 http://documentation.gabisoftware.com
DIN EN 15804:2012+A2:2019+AC:2021, Sustainability of
construction works - Environmental product declarations - Core IBU 2021
rules for the product category of construction products. Institut Bauen und Umwelt e.V.: General guidance for the EPD
program of the Institut Bauen und Umwelt e.V.. (IBU). Version
ISO 9001 2.0, Berlin: Institut Bauen und Umwelt e.V., 2021.
DIN EN ISO 9001:2015-11, Quality management systems - www.ibu-epd.com
Requirements.
Key to Steel
ISO 10270-1 Key to Steel (Stahlschlüssel) 2019, 25. edition, 2023, Verlag
DIN EN ISO 10270-1:2011, Steel wire for mechanical springs - Stahlschlüssel Wegst GmbH, Germany.
Part 1: Patented cold drawn unalloyed spring steel wire.
ökobaudat 2022
ISO 14001 ökobaudat 2022. EN 15804 and BNB compliant data for over
DIN EN ISO 14001:2015-11, Environmental management 700 building products.
systems - Requirements with guidance for use.
Ordinance on Biocide Products
ISO 14025 Regulation (EU) No 528/2012 of the European Parliament and
DIN EN ISO 14025:2011-10, Environmental labels and of the Council of 22 May 2012 concerning the making available
declarations - Type III environmental declarations - Principles on the market and use of biocidal products.
and procedures.
PCR Part A
ISO 14044 Product category rules for building-related products and
DIN EN ISO 14044:2006-10, Environmental management - Life services. Part A: Calculation rules for life cycle assessment and
cycle assessment - Requirements and guidance. project report requirements according to EN 15804+A2:2019.
Version 1.3. Berlin: Institut Bauen und Umwelt e.V.. (ed.), 2022.
ISO 45001
DIN EN ISO 45001:2018-03, Occupational health and safety PCR: Structural steels
management systems - Requirements with guidance for use. Product category rules for building-related products and
services. Part B: Requirements for the EPD for structural steels.
ISO 50001 Version v0. Berlin: Institut Bauen und Umwelt e.V., 08.03.2023.
DIN EN ISO 50001:2018-12, Energy management systems -
Requirements with guidance for use. worldsteel 2014
World Steel Association, February 14, 2014: A methodology to
Further references determine the LCI of steel industry co-products.
Candidate list worldsteel 2019
Candidate List of Substances of Very High Concern (ECHA World Steel Association, 2019: Life cycle inventory
Candidate List) of 16.01.2020, published in accordance with methodology report.
Article 59 (10) of the REACH Regulation Helsinki: European
8 Environmental Product Declaration - voestalpine Wire Austria GmbH - Shaped Wire
Publisher
Institut Bauen und Umwelt e.V. +49 (0)30 3087748- 0
Hegelplatz 1 info@ibu-epd.com
10117 Berlin www.ibu-epd.com
Germany
Programme holder
Institut Bauen und Umwelt e.V. +49 (0)30 3087748- 0
Hegelplatz 1 info@ibu-epd.com
10117 Berlin www.ibu-epd.com
Germany
Author of the Life Cycle Assessment
Daxner & Merl GmbH +43 676 849477826
Schleifmühlgasse 13/24 office@daxner-merl.com
1040 Wien www.daxner-merl.com
Austria
Owner of the Declaration
voestalpine AG +43/50304/15-0
voestalpine-Straße 3 info@voestalpine.com
4020 Linz www.voestalpine.com
Austria
9 Environmental Product Declaration - voestalpine Wire Austria GmbH - Shaped Wire
