ENVIRONMENTAL PRODUCT DECLARATION
as per ISO 14025 and EN 15804+A2
Owner of the Declaration Peiner Träger GmbH
Publisher Institut Bauen und Umwelt e.V. (IBU)
Programme holder Institut Bauen und Umwelt e.V. (IBU)
Declaration number EPD-PTR-20210292-CBA1-EN
Issue date 27.07.2023
Valid to 26.07.2028
Structural Steel - Beams and Sections
Peiner Träger GmbH
www.ibu-epd.com | https://epd-online.com
General Information
Peiner Träger GmbH Structural Steel - Beams and Sections
Programme holder Owner of the declaration
IBU – Institut Bauen und Umwelt e.V. Peiner Träger GmbH
Hegelplatz 1 Gerhard-Lucas-Meyer-Str. 10
10117 Berlin 31226 Peine
Germany Germany
Declaration number Declared product / declared unit
EPD-PTR-20210292-CBA1-EN 1 metric ton of structural steel beams and sections
This declaration is based on the product category rules: Scope:
Structural steels, 01.08.2021 This environmental product declaration (EPD) applies to hot rolled
(PCR checked and approved by the SVR) structural steel beams and sections produced by Peiner Träger GmbH, a
company of Salzgitter AG, at its only production site at Peine, Germany.
Information concerning SALCOS® (Salzgitter Low CO2 Steel) Structural
Issue date Steel - Beams and Sections are included in the Annex.
27.07.2023
The products are intended for the use in bolted, welded or otherwise
connected constructions of buildings, bridges and other structures. They
are produced via the electric arc furnace (EAF) route.
Valid to
The owner of the declaration shall be liable for the underlying information
26.07.2028 and evidence; the IBU shall not be liable with respect to manufacturer
information, life cycle assessment data and evidences.
The EPD was created according to the specifications of EN 15804+A2. In
the following, the standard will be simplified as EN 15804.
Verification
The standard EN 15804 serves as the core PCR
Independent verification of the declaration and data according to ISO
14025:2011
internally X externally
Dipl.-Ing. Hans Peters
(Chairman of Institut Bauen und Umwelt e.V.)
Florian Pronold Therese Daxner,
(Managing Director Institut Bauen und Umwelt e.V.) (Independent verifier)
1 Environmental Product Declaration - Peiner Träger GmbH - Structural Steel - Beams and Sections
Product
Performance data of the product in accordance with the
Product description/Product definition declaration of performance with respect to its essential
This EPD applies to 1 metric ton of hot rolled structural steel characteristics according to EN 10025-1.
beams and sections in structural steel grades. For the placing Additional information can be obtained from www.peiner-
on the market of the product in the European Union/European traeger.de.
Free Trade Association (EU/EFTA) (with the exception of
Switzerland) Regulation (EU) No. 305/2011 (CPR) applies. The Base materials/Ancillary materials
product needs a declaration of performance taking into Structural steels are non-alloyed or low-alloyed iron alloys with
consideration EN 10025-1 and the CE-marking. For the a carbon content of typically below 0.3%. The base material for
application and use the respective national provisions apply. structural steel beams and sections of this EPD is steel scrap,
which is recycled by the EAF-steelmaking process.
Application
Structural steel beams and sections are intended for the use in Alloying elements like manganese, silicon, aluminum and
bolted, welded or otherwise connected constructions of vanadium are added in the form of ferroalloys or metals.
buildings, bridges and other structures, or in composite steel The rates of these additives depend on the steel grade and are
and concrete structures. on average: 0,9% silico manganese, 0,2% ferro manganese,
Examples are: 0,1% ferro silicon, 0,1% aluminium and < 0,1% other alloys (e.
• buildings (industrial and storage buildings, residual and g. ferro vanadium, ferro niobium, ferro titanium).
office buildings, stadiums, airports, train stations, car
parks, convention centers, etc.) Other elements such as nitrogen or copper may be present in
• bridges (railway bridges, road bridges, pedestrian the steel depending on the steel grade, but are generally not
bridges, etc.) intentionally added.
• other structures (industrial and power plants, onshore
and offshore energy facilities, harbour and port The product for authorization contains substances on the
constructions, etc.) ECHA list of substances of very high concern (SVHC) (14 July
2021) above 0.1 % by mass: No.
Technical Data
This EPD is valid for structural steel beams and sections of The product contains further carcinogenic, mutagenic,
various steel grades and different forms of delivery. Specific reprotoxic (CMR) substances of category 1A or 1B that not in
information on steel grades, dimensions and tolerances can be the candidate list, above 0.1 mass % in at least one
found in the relevant literature and/or standards. subproduct: No.
In Europe the most relevant standards applicable for structural
steel beams and sections are EN 10025 and EN 10365 in Biocides have been added to the construction product, or the
combination with EN 10034 or EN 10279. Also international product has been treated with biocides (a treated product
product standards like ASTM A6, ASTM A36, ASTM A992, pursuant to the Biocidal Product Regulation (EU) No.
ASTM A572, etc. can be applicable. 528/2012): No.
Constructional data Reference service life
Name Value Unit A reference service life for structural steel beams and sections
Density 7850 kg/m3 is not declared. These are construction products with many
Modulus of elasticity 210000 N/mm2 different applications purposes that define the service life of the
construction and their components.
Coefficient of thermal expansion 12 10-6K-1
Thermal conductivity 48 W/(mK)
Melting point (depending on the alloy
1536 °C
proportions up to)
Shear modulus 81000 N/mm²
LCA: Calculation rules
For the calculation of the declared average, all grades
Declared Unit produced were included in the form of an annual average. Input
The reference unit is 1 ton of structural steel beams and and production quantities for the entire calendar year 2020
sections. were taken into account. The calculated results can thus be
Foreground data for the production are integrated into the LCA considered representative for the entire product portfolio
FE (GaBi) Software model for the production site under study. structural steels – beams and sections of Peiner Träger GmbH.
LCI is assessed as per the annual production data of Peiner
Träger GmbH at the site Peine. The EPD is calculated with residual grid mix.
Background data are taken from the LCA FE (GaBi) Database. System boundary
Type of the EPD: cradle-to-gate - with options: Module A1-A3,
Declared unit
Modules C1-C4 and Module D were
Name Value Unit
considered.
Declared unit 1 t
Density 7850 kg/m3 Modules A1-A3 covers the production stage including the
upstream burdens of purchased raw materials (ferro-alloys,
Conversion factor to 1 kg 1000 -
lime, dolomite, etc.), their transports and the manufacturing at
2 Environmental Product Declaration - Peiner Träger GmbH - Structural Steel - Beams and Sections
the production site in Peine. Module D refers to the End-of-Life, including recycling and/or
Material and energy flows for the electric arc furnace and the reuse.
hot rolling mills are considered.
Electricity consumption is modelled via residual grid mix (i.e. Geographic Representativeness
production in Germany + imports - exports - certified "green" Land or region, in which the declared product system is
electricity). manufactured, used or handled at the end of the product´s
lifespan: Germany
Modules C1-C4 consider the dismantling of the considered
product (C1), the transportation of the dismantled components
Comparability
to their final EoL destination (C2), the waste processing for
Basically, a comparison or an evaluation of EPD data is only
reuse, recovery or recycling (C3) as well as the disposal (C4).
possible if all the data sets to be compared were created
It is assumed that the product is not connected with other
according to EN 15804 and the building context, respectively
materials and can therefore be dismantled. Associated efforts
the product-specific characteristics of performance, are taken
are negligible, no environmental impacts from the
into account. The LCA FE (GaBi) background database
deconstruction of the products are declared (Module C1)
(content version 2022.2) was used to calculate the LCA.
LCA: Scenarios and additional technical information
technical scenario information for Module A5.
Characteristic product properties of biogenic carbon
End of life (C1 - C4)
The declared product does not include biogenic carbon.
Name Value Unit
There is no packaging considered within the given study. Landfilling - Scenario 0 0 kg
Landfilling - Scenario 1 0 kg
The EPD covers four End of Life scenarios (SteelConstruction-
Landfilling - Scenario 2 1000 kg
info; Sansom, M. / Meijer, J.):
Landfilling - Scenario 3 10 kg
• Scenario 0: 100% Recycling Reuse, recovery and/or recycling potentials (D), relevant
• Scenario 1: 100% Reuse scenario information
• Scenario 2: 100% Loss / Landfill Name Value Unit
• Scenario 3: 88% Recycling, 11% Reuse and 1% Loss
Recycling - Scenario 0 1000 kg
Recycling - Scenario 1 0 kg
The following technical information is a basis for the declared
modules or can be used for developing specific scenarios in the Recycling - Scenario 2 0 kg
context of a building assessment if modules are not declared Recycling - Scenario 3 880 kg
(MND). Reuse - Scenario 0 0 kg
Reuse - Scenario 1 1000 kg
A5 is not declared including the disposal of the packaging
Reuse - Scenario 2 0 kg
material on the construction site, the amounts of packaging
materials included in the LCA calculations must be declared as Reuse - Scenario 3 110 kg
3 Environmental Product Declaration - Peiner Träger GmbH - Structural Steel - Beams and Sections
LCA: Results
The following table contains the LCA results for a declared unit of 1 ton structural steel beams and sections.
DESCRIPTION OF THE SYSTEM BOUNDARY (X = INCLUDED IN LCA; ND = MODULE OR INDICATOR NOT DECLARED; MNR =
MODULE NOT RELEVANT)
Benefits and
Construction loads beyond
Product stage Use stage End of life stage
process stage the system
boundaries
la ire ta m w a Ry lp p u s tro p s n a rT g n iru tc a fu n a M e h t m o rf tro p s n a rTe tis e h t o t e ta g y lb m e s s A e s U e c n a n e tn ia M ria p e R tn e m e c a lp e R tn e m h s ib ru fe R y g re n e la n o ita re p Oe s u re ta w la n o ita re p Oe s u n o itc u rts n o c -e Dn o itilo m e d tro p s n a rT g n is s e c o rp e ts a W la s o p s iD -e s u e R-y re v o c e R-g n ilc y c e Rla itn e to p
A1 A2 A3 A4 A5 B1 B2 B3 B4 B5 B6 B7 C1 C2 C3 C4 D
X X X MND MND MND MND MNR MNR MNR MND MND X X X X X
RESULTS OF THE LCA - ENVIRONMENTAL IMPACT according to EN 15804+A2: 1 ton structural steel beams and sections
Parameter Unit A1-A3 C1 C2 C3 C3/1 C3/2 C3/3 C4 C4/1 C4/2 C4/3 D D/1 D/2 D/3
6.88E 5.41E -6.87E 1.97E
GWP-total kg CO 2 eq +02 0 +00 0 0 0 0 0 0 1.45E+01 1.45E-01 2.36E+02 +02 +03 1.52E+02
6.88E 5.15E -6.87E 1.97E
GWP-fossil kg CO 2 eq +02 0 +00 0 0 0 0 0 0 1.49E+01 1.49E-01 2.36E+02 +02 +03 1.52E+02
GWP- -1.01E
biogenic kg CO 2 eq 6.2E-01 0 2.66E-01 0 0 0 0 0 0 -4.42E-01-4.42E-03-1.21E-01-6.18E-01 +00 -1.84E-01
GWP-luluc kg CO 2 eq7.38E-02 0 0 0 0 0 0 0 0 2.75E-02 2.75E-04 4.88E-03 -7.05E-024.06E-02-3.06E-03
kg CFC11
ODP 1.07E-09 0 0 0 0 0 0 0 0 3.51E-11 3.51E-13 5.17E-13 -1.07E-09 4.3E-12 -1.17E-10
eq
4.23E
AP mol H+ eq 1.7E+00 0 2.15E-03 0 0 0 0 0 0 1.06E-01 1.06E-03 5.08E-01 -1.7E+00 3.02E-01
+00
EP-
kg P eq 1.1E-04 0 0 0 0 0 0 0 0 2.53E-05 2.53E-07 4.29E-05 -1.07E-043.57E-04 2.95E-05
freshwater
EP-marine kg N eq 4.65E-01 0 1.08E-03 0 0 0 0 0 0 2.71E-02 2.71E-04 8.93E-02 -4.64E-017.44E-01 3.5E-02
5.09E -5.07E 6.53E
EP-terrestrial mol N eq 0 1.21E-02 0 0 0 0 0 0 2.97E-01 2.97E-03 7.84E-01 1.97E-01
+00 +00 +00
kg
1.29E -1.29E 3.02E
POCP NMVOC 0 2.2E-03 0 0 0 0 0 0 8.22E-02 8.22E-04 3.62E-01 2.07E-01
+00 +00 +00
eq
ADPE kg Sb eq 1.18E-04 0 0 0 0 0 0 0 0 1.53E-06 1.53E-08 5.89E-04 -1.18E-044.91E-03 5.55E-04
9.05E -9.04E 1.81E
ADPF MJ 0 0 0 0 0 0 0 0 1.95E+021.95E+002.17E+03 1.1E+03
+03 +03 +04
m3 world
7.24E -7.23E 3.66E
WDP eq 0 0 0 0 0 0 0 0 1.64E+00 1.64E-02 4.39E+01 3.44E+01
+01 +01 +02
deprived
GWP = Global warming potential; ODP = Depletion potential of the stratospheric ozone layer; AP = Acidification potential of land and water; EP =
Eutrophication potential; POCP = Formation potential of tropospheric ozone photochemical oxidants; ADPE = Abiotic depletion potential for non-fossil
resources; ADPF = Abiotic depletion potential for fossil resources; WDP = Water (user) deprivation potential)
RESULTS OF THE LCA - INDICATORS TO DESCRIBE RESOURCE USE according to EN 15804+A2: 1 ton structural steel
beams and sections
Parameter Unit A1-A3 C1 C2 C3 C3/1 C3/2 C3/3 C4 C4/1 C4/2 C4/3 D D/1 D/2 D/3
4.32E -1.37E -4.29E -1.14E -1.79E
PERE MJ 0 1.89E+00 0 0 0 0 0 0 2.93E+012.93E-01
+02 +02 +02 +03 +02
PERM MJ 0 0 0 0 0 0 0 0 0 0 0 0 0 0 0
4.32E -1.37E -4.29E -1.14E -1.79E
PERT MJ 0 1.89E+00 0 0 0 0 0 0 2.93E+012.93E-01
+02 +02 +02 +03 +02
9.05E -9.04E
PENRE MJ 0 3.33E+01 0 0 0 0 0 0 1.96E+021.96E+002.17E+03 1.81E+04 1.1E+03
+03 +03
PENRM MJ 0 0 0 0 0 0 0 0 0 0 0 0 0 0 0
9.05E -9.04E
PENRT MJ 0 3.33E+01 0 0 0 0 0 0 1.96E+021.96E+002.17E+03 1.81E+04 1.1E+03
+03 +03
1.14E -1.37E -1.14E -1.31E
SM kg 0 0 0 0 0 0 0 0 0 0 0
+03 +02 +03 +02
RSF MJ 0 0 0 0 0 0 0 0 0 0 0 0 0 0 0
NRSF MJ 0 0 0 0 0 0 0 0 0 0 0 0 0 0 0
2.67E -2.67E
FW m3 0 2.14E-03 0 0 0 0 0 0 4.97E-02 4.97E-04 9.92E-01 8.26E+006.63E-01
+00 +00
PERE = Use of renewable primary energy excluding renewable primary energy resources used as raw materials; PERM = Use of renewable primary
energy resources used as raw materials; PERT = Total use of renewable primary energy resources; PENRE = Use of non-renewable primary energy
excluding non-renewable primary energy resources used as raw materials; PENRM = Use of non-renewable primary energy resources used as raw
materials; PENRT = Total use of non-renewable primary energy resources; SM = Use of secondary material; RSF = Use of renewable secondary fuels;
NRSF = Use of non-renewable secondary fuels; FW = Use of net fresh water
4 Environmental Product Declaration - Peiner Träger GmbH - Structural Steel - Beams and Sections
RESULTS OF THE LCA – WASTE CATEGORIES AND OUTPUT FLOWS according to EN 15804+A2:
1 ton structural steel beams and sections
Parameter Unit A1-A3 C1 C2 C3 C3/1 C3/2 C3/3 C4 C4/1 C4/2 C4/3 D D/1 D/2 D/3
HWD kg 8.86E-07 0 1.6E-10 0 0 0 0 0 0 1E-08 1E-10 1.68E-08 -8.86E-07 1.4E-07 -8.13E-08
7.19E -3.29E -7.19E -2.74E -3.25E
NHWD kg 0 4.78E-03 0 0 0 0 0 0 1E+03 1E+01
+00 +01 +00 +02 +01
RWD kg 4.99E-01 0 4.1E-05 0 0 0 0 0 0 2.17E-03 2.17E-05 -2.7E-04 -4.98E-01-2.25E-03-5.51E-02
CRU kg 0 0 0 0 1E+03 0 1.1E+02 0 0 0 0 0 0 0 0
MFR kg 0 0 0 1E+03 0 0 8.8E+02 0 0 0 0 0 0 0 0
MER kg 0 0 0 0 0 0 0 0 0 0 0 0 0 0 0
EEE MJ 0 0 0 0 0 0 0 0 0 0 0 0 0 0 0
EET MJ 0 0 0 0 0 0 0 0 0 0 0 0 0 0 0
HWD = Hazardous waste disposed; NHWD = Non-hazardous waste disposed; RWD = Radioactive waste disposed; CRU = Components for re-use;
MFR = Materials for recycling; MER = Materials for energy recovery; EEE = Exported electrical energy; EET = Exported thermal energy
RESULTS OF THE LCA – additional impact categories according to EN 15804+A2-optional:
1 ton structural steel beams and sections
Parameter Unit A1-A3 C1 C2 C3 C3/1 C3/2 C3/3 C4 C4/1 C4/2 C4/3 D D/1 D/2 D/3
Disease
PM ND ND ND ND ND ND ND ND ND ND ND ND ND ND ND
incidence
kBq U235
IR ND ND ND ND ND ND ND ND ND ND ND ND ND ND ND
eq
ETP-fw CTUe ND ND ND ND ND ND ND ND ND ND ND ND ND ND ND
HTP-c CTUh ND ND ND ND ND ND ND ND ND ND ND ND ND ND ND
HTP-nc CTUh ND ND ND ND ND ND ND ND ND ND ND ND ND ND ND
SQP SQP ND ND ND ND ND ND ND ND ND ND ND ND ND ND ND
PM = Potential incidence of disease due to PM emissions; IR = Potential Human exposure efficiency relative to U235; ETP-fw = Potential comparative
Toxic Unit for ecosystems; HTP-c = Potential comparative Toxic Unit for humans (cancerogenic); HTP-nc = Potential comparative Toxic Unit for humans
(not cancerogenic); SQP = Potential soil quality index
Disclaimer 1 – for the indicator “Potential Human exposure efficiency relative to U235”. This impact category deals mainly with the
eventual impact of low-dose ionizing radiation on human health of the nuclear fuel cycle. It does not consider effects due to possible
nuclear accidents, occupational exposure or radioactive waste disposal in underground facilities. Potential ionizing radiation from the
soil, radon and from some construction materials is also not measured by this indicator.
Disclaimer 2 – for the indicators “abiotic depletion potential for non-fossil resources”, “abiotic depletion potential for fossil resources”,
“water (user) deprivation potential, deprivation-weighted water consumption”, “potential comparative toxic unit for ecosystems”,
“potential comparative toxic unit for humans – cancerogenic”, “Potential comparative toxic unit for humans - not cancerogenic”,
“potential soil quality index”. The results of this environmental impact indicator shall be used with care as the uncertainties on these
results are high as there is limited experience with the indicator.
References
Standards EN 10025-3:2019 Hot rolled products of structural steels – Part
3: Technical delivery conditions for normalized/normalized
ASTM A6 rolled weldable fine grain structural steels
ASTM A6 / A6M - 19 Standard Specification for General
Requirements for Rolled Structural Steel Bars, Plates, Shapes, EN 10025-4
and Sheet Piling EN 10025-4:2019 Hot rolled products of structural steels – Part
4: Technical delivery conditions for thermomechanical rolled
ASTM A36 weldable fine grain structural steels
ASTM A36 / A36M - 19 Standard Specification for Carbon
Structural Steel EN 10025-5
EN 10025-5:2019 Hot rolled products of structural steels – Part
ASTM A572 5: Technical delivery conditions for structural steels with
ASTM A572 / A572M - 21e1 Standard Specification for High- improved atmospheric corrosion resistance
Strength Low-Alloy Columbium-Vanadium Structural Steel
EN 10034
ASTM A992 EN 10034:1993 Structural steel I and H sections; Tolerances on
ASTM A992 / A992M - 20 Standard Specification for Structural shape and dimensions
Steel Shapes
EN 10279
EN 10025-1 EN 10279:2000 Hot rolled steel channels - Tolerances on
EN 10025-1:2004 Hot rolled products of structural steels – Part shape, dimensions and mass
1: General technical delivery conditions
EN 10365
EN 10025-2 EN 10365:2017 Hot rolled steel channels, I and H sections -
EN 10025-2:2019 Hot rolled products of structural steels – Part Dimensions and masses
2: Technical delivery conditions for non-alloy structural steels
EN 15804
EN 10025-3 EN 15804:2019+A2, Sustainability of construction works —
5 Environmental Product Declaration - Peiner Träger GmbH - Structural Steel - Beams and Sections
Environmental Product Declarations — Core rules for the IBU 2021, General Instructions for the EPD programme of
product category of construction products Institut Bauen und Umwelt e.V. Version 2.0, Berlin: Institut
Bauen und Umwelt e.V., 2021, www.ibu-epd.de
ISO 14025
DIN EN ISO 14025:2011-10, Environmental labels and PCR, Part A
declarations — Type III environmental declarations —
Principles and procedures Product Category Rules for Building-Related Products and
Services, Calculation Rules for the Life Cycle Assessment and
Further References Requirements on the Project Report. Institut Bauen und Umwelt
e.V. (IBU), 2021, www.bau-umwelt.de
Candidate List of SVHC
Candidate List of substances of very high concern for PCR, Part B
Authorisation (published by the European Chemicals Agency Requirements on the EPD for Structural steels – Institut Bauen
(ECHA) in accordance with Article 59(10) of the REGULATION und Umwelt e.V., Königswinter (pub.): From the range of
(EC) No 1907/2006 OF THE EUROPEAN PARLIAMENT AND Environmental Product Declarations of Institute Construction
OF THE COUNCIL of 18 December 2006 concerning the and Environment e.V. (IBU), 2019
Registration, Evaluation, Authorisation and Restriction of
Chemicals (REACH)) Sansom, M. / Meijer, J.
Life-cycle assessment (LCA) for steel construction, Ascot,
LCA FE (GaBi) Software / Database Culemborg. 2002
GaBi, Software and Database for Life Cycle Engineering,
Sphera Solution GmbH, Leinfelden-Echterdingen, 2022, SteelConstruction-info
http://documentation.gabi-software.com https://www.steelconstruction.info/The_recycling_and_reuse_survey
IBU 2021
6 Environmental Product Declaration - Peiner Träger GmbH - Structural Steel - Beams and Sections
Publisher
Institut Bauen und Umwelt e.V. +49 (0)30 3087748- 0
Hegelplatz 1 info@ibu-epd.com
10117 Berlin www.ibu-epd.com
Germany
Programme holder
Institut Bauen und Umwelt e.V. +49 (0)30 3087748- 0
Hegelplatz 1 info@ibu-epd.com
10117 Berlin www.ibu-epd.com
Germany
Author of the Life Cycle Assessment
Sphera Solutions GmbH +49 711 341817-0
Hauptstraße 111- 113 info@sphera.com
70771 Leinfelden-Echterdingen www.sphera.com
Germany
Owner of the Declaration
Peiner Träger GmbH +49 51 71 91-01
Gerhard-Lucas-Meyer-Str. 10 peiner.traeger@salzgitter-ag.de
31226 Peine www.peiner-traeger.de
Germany
7 Environmental Product Declaration - Peiner Träger GmbH - Structural Steel - Beams and Sections
