ENVIRONMENTAL PRODUCT DECLARATION
as per ISO 14025 and EN 15804+A1
Owner of the Declaration Etex Building Performance International
Programme holder Institut Bauen und Umwelt e.V. (IBU)
Publisher Institut Bauen und Umwelt e.V. (IBU)
Declaration number EPD-PMT-20210295-IBC1-EN
Issue date 23.11.2021
Valid to 22.11.2026
PROMATECT®-LS
Medium density calcium silicate fire protective boards
Promat
www.ibu-epd.com | https://epd-online.com
Umwelt Produktdeklaration Name des Herstellers – Name des Produkts
1. General Information
Etex Building Performance NV PROMATECT®-LS
Programme holder Owner of the declaration
IBU – Institut Bauen und Umwelt e.V. Etex Building Performance International
Panoramastr. 1 500 Rue Marcel Demonque
10178 Berlin F-84915 Avignon
Germany France
Declaration number Declared product / declared unit
EPD-PMT-20210295-IBC1-EN The functional unit is 1 m² of PROMATECT®-LS with a
thickness of 35 mm.
This declaration is based on the product Scope:
category rules: The life cycle assessment is based on production data
Calcium silicate insulating materials, 11.2017 of PROMATECT®-LS of the year 2019 at the
(PCR checked and approved by the SVR) production site Tisselt, Belgium.
Issue date The owner of the declaration shall be liable for the
23.11.2021 underlying information and evidence; the IBU shall not
be liable with respect to manufacturer information, life
cycle assessment data and evidences.
Valid to
The EPD was created according to the specifications
22.11.2026
of EN 15804+A1. In the following, the standard will be
simplified as EN 15804.
Verification
The standard EN 15804 serves as the core PCR
Independent verification of the declaration and data
according to ISO 14025:2010
Dipl. Ing. Hans Peters internally x externally
(chairman of Institut Bauen und Umwelt e.V.)
Dr. Alexander Röder Vito D'Incognito
(Managing Director Institut Bauen und Umwelt e.V.)) (Independent verifier)
2. Product
2.1 Product description/Product definition
PROMATECT®-LS is a lightweight, non-combustible, Constructional data
fire-resisting calcium silicate board, not sensitive to Name Value Unit
moisture. Gross density according to ETA 460 -
kg/m3
11/0039 620
For the placing of the product on the market in the Compressive strength according to
4.2 N/mm2
European Union/European Free Trade Association ETA 11/0039
EU/EFTA (with the exception of Switzerland) the Tensile strength (perpendicular)
0.056 N/mm2
Regulation (EU) No. 305/2011 (CPR) applies. The according to EN 1607
product needs a declaration of performance taking into Flexural strength according to ETA
1.5 N/mm2
consideration ETA 11/0039_2018-04-12 and the CE- 11/0039
marking. For the application and use the respective Thermal conductivity according to ETA
0.087 W/(mK)
national provisions apply. 11/0039
Water vapour diffusion resistance
3.9 -
factor according to EN 12572
2.2 Application Tensile strength (parallel) according to
PROMATECT®-LS is primarily used in interior building EN 1608 445 kPa
applications where normal to high levels of fire
Values are guidance values and do not reflect a
resistance are required.
statistical evaluation or guaranteed value.
PROMATECT®-LS is intended to protect elements or
to be used in technical services assemblies.
Performance data of the product in accordance with
Main application areas are the fire protection of ducts
the declaration of performance with respect to its
such as cable, ventilation and smoke extraction ducts.
essential characteristics according to ETA 11/0039.
2.3 Technical Data
2 Environmental Product Declaration Etex Building Performance NV – PROMATECT®-LS
2.4 Delivery status 2.8 Product processing/Installation
PROMATECT®-LS fire protective calcium silicate The fire protective board is cut and machined using
boards are 1200 x 2500 mm and are delivered in conventional woodworking equipment.
various thicknesses: 30,35,40,45 and 50 mm. Fixing the boards will require appropriate means,
which will depend upon the application and bearing
2.5 Base materials/Ancillary materials structure. Boards can be installed using screws or
The following raw materials expressed in weight glues.
percentages are used to produce PROMATECT®-LS: Industrial and environmental protection are assured
- sand: 25-45 % through training and coaching staff on safety and
- lime: 25-45 % environmental impacts. Dust levels are kept low by
- cement: <15 % performing dust extraction. Noise is reduced by noise
- fibres: <6 % insulation on the machines and ear protection is
Reaction is performed in an aqueous suspension. provided for persons entering the production area.
Regular measurements on noise and dust are
This article contains substances listed in the candidate performed and show conformity to the permitted
list (date: 19.01.2021) exceeding 0.1 percentage by levels.
mass: no. All national, local and other applicable safety
This article contains other carcinogenic, mutagenic, regulations are complied with.
reprotoxic (CMR) substances in categories 1A or 1B
which are not on the candidate list, exceeding 0.1 2.9 Packaging
percentage by mass: no. All fire protection boards are packed onto wooden
Biocide products were added to this construction pallets, wrapped with polyester strapping tape and
product or it has been treated with biocide products strengthened with cardboard corners.
(this then concerns a treated product as defined by the
(EU) Ordinance on Biocide Products No. 528/2012):
no. 2.10 Condition of use
PROMATECT®-LS boards are resistant to the effects
of moisture and will not physically deteriorate when
2.6 Manufacture used in damp or humid conditions. Performance
Sand, water and lime are mixed and blended in a characteristics are not degraded by age or moisture.
reactor to form calcium silicate. This is combined in a Boards do not encourage mould growth and are
mixer with the other raw materials to form a thick resistant to attacks by insects or vermin.
slurry. The slurry is formed to a board in a filter press.
Boards are dried, edges are trimmed and the upper 2.11 Environment and health during use
surface is sanded to the specific thickness. All material PROMATECT®-LS is chemically inert. When the
which is cut off or sanded away is fully recycled within product is used as designed, the current state of
the process. knowledge indicates that there is no risk involved for
the environment or health.
2.12 Reference service life
The service life according to the "Bundesinstitut für
Bau-, Stadt- und Raumforschung" (BBSR) table is
indicated to be ≥ 50 years.
The reference service life (RSL) is therefore estimated
to be 50 years. This RSL corresponds to the period
after which a building renovation is usually needed,
independently of the actual lifetime of the product
(which can be longer than 50 years).
2.13 Extraordinary effects
Fire
The PROMATECT®-LS boards have a reaction to fire
The quality management system of the company and
classification A1 or non-combustible according to
the production facility are certified according to ISO
EN13501-1.
9001.
Fire protection
Name Value
2.7 Environment and health during
Building material class A1
manufacturing
Burning droplets /
Promat commits to a clean, healthy and safe working
Smoke gas development /
environment for every person working in and for the
company.
Water
The company and the manufacturing site have an
All ingredients are firmly bound in the matrix. The
environment, health and safety management system
boards are insensitive to moisture and no ingredients
which is ISO 14001 and ISO 45001 certified. The
which could be hazardous to water are washed out in
manufacturing plant adheres to the Belgium
the event of extraordinary effects by water.
environmental and health and safety regulations.
3 Environmental Product Declaration Etex Building Performance NV – PROMATECT®-LS
Mechanical destruction For this EPD, a conservative worst-case scenario was
In order to prevent any reduction of fire performance chosen at the end-of-life stage and the product was
following unforeseeable mechanical destruction, all sent for 100% to landfill.
damage of the components needs to be repaired using
materials specified by the ETA 11/0039. 2.15 Disposal
Besides the need for repair, the destruction will not Within the production process, generated waste is
have any significant environmental impact. immediately re-used within the process.
When after end-of-life re-using or recycling the boards
2.14 Re-use phase as described in the previous paragraph is not practical,
Several possibilities exist for the boards after the end- the boards can be disposed to landfill without pre-
of-life of the application in which they were used. treatment thanks to the largely mineral ingredients
If the boards are removed non-destructively by resulting in an inert matrix, The waste code in
releasing the screws, the undamaged product can be accordance with the European List of Waste is
re-used in accordance with the original purpose. 170904.
If not contaminated with other building construction
material, the boards also allow being recycled by the 2.16 Further information
manufacturer. Further information is available on the following web
Furthermore, the products referred to could be used as site :
filler and bulk material in civil engineering, as an https://www.promat.com
absorber in cat litter or be recycled in the cement
industry.
3. LCA: Calculation rules
3.1 Declared Unit  production of packaging
The declared unit is 1 m² PROMATECT®-LS with a
thickness of 35 mm.
The results for other thicknesses can be obtained by
Construction stage (A4-A5):
multiplying the presented results by the corresponding
 transportation of product to the construction
adjustment factor as included in the table.
site
 disposal of installation wastes
Declared unit  incineration of packaging materials (potential
Name Value Unit
benefits from energy substitution within the
Gross density 502 kg/m3
incineration process are declared in module
Declared unit 1.00 m²
D)
Grammage 17.6 kg/m²
Conversion factor to 1 kg (divide
results by this factor to obtain the 17.6 -
results for 1 kg) Use stage (B1-B7):
Adjustment factor to 1 ton  efforts for the use of the product,
(multiply results by this factor to 56.82 - maintenance and operational efforts
obtain the results for 1 ton)
 modules B3, B4, B5 are declared as MNR
Adjustment factor to 1 m² 30 mm
(module not relevant) according to the IBU
(multiply results by this factor to 0.86 -
requirement. These modules are defined on
obtain the results for 1 m² 30 mm)
Adjustment factor to 1 m² 40 mm building level in general
(multiply results by this factor to 1.14 -
obtain the results for 1 m² 40 mm)
Adjustment factor to 1 m² 45 mm End-of-life stage (C1-C4):
(multiply results by this factor to 1.29 -  transport to disposal of the material
obtain the results for 1 m² 45 mm)
 landfill end-of-life scenario was considered
Adjustment factor to 1 m² 50 mm
(multiply results by this factor to 1.43 -
obtain the results for 1 m² 50 mm)
Loads and benefits beyond system boundary (D):
 loads and benefits from the recycling of
production waste and incineration of
3.2 System boundary packaging waste
Type of the EPD: cradle to grave.
The following life cycle stages and modules are
included:
3.3 Estimates and assumptions
Production stage (A1-A3): Most of the input and output influences of the Life
Cycle Inventory Analysis could be depicted using
 pre-chains of the raw materials and their
corresponding data from the GaBi database.
transportation to the manufacturing site
Assumptions and approximations were applied in case
 energy consumption during production
of a lack of representative data.
 recycling and disposal of production wastes
4 Environmental Product Declaration Etex Building Performance NV – PROMATECT®-LS
There were no data records in the GaBi database 3.7 Period under review
available for the wooden pallets, they were Data for the entire production period of 2019 were
approximated using the "Solid construction timber" collected and used for this EPD.
dataset.
The waste water treatment of process water was 3.8 Allocation
approximated by datasets of municipal waste water Allocation in background data
treatment, which will result in an overestimation of Specific information on allocation within the
impacts. background data is given in the GaBi documentation.
All assumptions and approximations were documented Allocation in foreground data
precisely. The production process does not deliver any co-
products. In modules A1 to A3, specific raw material
3.4 Cut-off criteria and transport data were available, energy, waste and
In the assessment, all utilised raw material, thermal water could not be directly allocated to the product and
energy and electric power were considered were allocated via the production volume of the
using GaBi datasets. Only the transport of packaging, specific products.
production waste to recycling/disposal and of Allocation for waste materials
installation loss waste to recycling was cut-off in this The environmental burden of the incineration of
study. packaging in the construction process stage is
Production of capital equipment, facilities and assigned to the system (A5); resulting credits for
infrastructure required for the manufacture are outside thermal and electrical energy are declared in module
the scope of the study and thus were not included. D.
3.5 Background data
Background data were sourced from GaBi 10 database 3.9 Comparability
version 2021. Basically, a comparison or an evaluation of EPD data
is only possible if all the data sets to be compared
3.6 Data quality were created according to EN 15804 and the building
This study is mainly based on primary data collected context, respectively the product-specific
directly from the manufacturing site and therefore data characteristics of performance, are taken into account.
quality can be assumed to be very good.
The last update of the GaBi database used for GaBi database version 2021.1 serves as a
the background data was February 2021. background database for the calculation of the life
cycle assessment.
4. LCA: Scenarios and additional technical information
Name Value Unit
Information on maintenance - -
Transport to the building site (A4) Number/
Maintenance cycle -
For the transport from the factory gate to the building RSL
site, an average distance of 100km was assumed. This Water consumption - m3
distance can be assumed to be representative of Auxiliary - kg
deliveries within Belgium. Other resources - kg
Name Value Unit Electricity consumption - kWh
Litres of fuel 0.037 l/100km Other energy carriers - MJ
Transport distance 100 km Material loss - kg
Capacity utilisation (including empty
61 %
runs)
Repair (B3)
Gross density of products transported 502 kg/m3 Name Value Unit
Information on the repair process - -
Information on the inspection process - -
Installation into the building (A5) Number/
Only waste treatment of installation loss and packaging Repair cycle - RSL
is considered in this module.
Water consumption - m3
Auxiliary - kg
Installation into the building (A5)
Other resources - kg
Name Value Unit
Electricity consumption - kWh
Material loss 0.88 kg
Other energy carriers - MJ
VOC in the air 0 kg
Material loss - kg
Replacement (B4) / Refurbishment (B5)
Use or application of the installed product (B1) see
Name Value Unit
section 2.12 "Use"
Number/
No efforts and releases of substances occur during the Replacement cycle -
RSL
normal (i.e. anticipated) use phase.
Electricity consumption - kWh
Name Value Unit
Litres of fuel - l/100km
Maintenance (B2) Replacement of worn parts - kg
No efforts occur during maintenance.
5 Environmental Product Declaration Etex Building Performance NV – PROMATECT®-LS
Reference service life
Name Value Unit
Reference service life - a
Life Span (according to BBSR) >=50 a
Life Span according to the
- a
manufacturer
Declared product properties (at the
- -
gate) and finishes
Design application parameters (if
instructed by the manufacturer),
including the references to the - -
appropriate practices and application
codes
An assumed quality of work, when
installed in accordance with the - -
manufacturer’s instructions
Outdoor environment, (for outdoor
applications), e.g. weathering,
pollutants, UV and wind exposure, - -
building orientation, shading,
temperature
Indoor environment (for indoor
applications), e.g. temperature, - -
moisture, chemical exposure
Usage conditions, e.g. frequency of
- -
use, mechanical exposure
Maintenance e.g. required frequency,
type and quality and replacement of - -
components
Operational energy use (B6) and Operational water
use (B7)
No efforts occur in modules B6 and B7.
Name Value Unit
Water consumption - m3
Electricity consumption - kWh
Other energy carriers - MJ
Equipment output - kW
End-of-life (C1-C4)
A conservative approach was used in this study.
Although after end-of-life, scenarios, where the
boards are re-used or recycled, are realistic, a
scenario with 100% landfill was used.
Name Value Unit
Landfilling 17.6 kg
Re-use, recovery and/or recycling potentials (D),
relevant scenario information
Although re-use and recycling of the PROMATECT®-
LS is possible, this is not yet a widely established
practice. Therefore, no possible benefits of recycling or
re-use of the boards were taken into account in this
study. In module D, only the benefits from the recycling
of production waste and incineration of waste
packaging were taken into account.
Name Value Unit
Exported electrical energy 2.09 MJ
Exported thermal energy 3.77 MJ
6 Environmental Product Declaration Etex Building Performance NV – PROMATECT®-LS
5. LCA: Results
The following tables depict the results of the indicators for the Life Cycle Assessment, use of resources and waste
with reference to 1 m² of PROMATECT®-LS with a thickness of 35 mm.
DESCRIPTION OF THE SYSTEM BOUNDARY (X = INCLUDED IN LCA; MND = MODULE NOT DECLARED;
MNR = MODULE NOT RELEVANT)
BENEFITS AND
CONSTRUCTI LOADS
PRODUCT STAGE ON PROCESS USE STAGE END OF LIFE STAGE BEYOND THE
STAGE SYSTEM
BOUNDARIES
7 Environmental Product Declaration Etex Building Performance NV – PROMATECT®-LS
lairetam
waR
ylppus tropsnarT
gnirutcafunaM
eht
morf
tropsnarT
etis
eht
ot
etag
ylbmessA esU
ecnanetniaM
riapeR
tnemecalpeR tnemhsibrufeR
ygrene
lanoitarepO esu
retaw
lanoitarepO esu
noitcurtsnoc-eD
noitilomed tropsnarT
gnissecorp
etsaW
lasopsiD -esueR -yrevoceR -gnilcyceR laitnetop
A1 A2 A3 A4 A5 B1 B2 B3 B4 B5 B6 B7 C1 C2 C3 C4 D
X X X X X X X MNR MNR MNR X X X X X X X
RESULTS OF THE LCA - ENVIRONMENTAL IMPACT according to EN 15804+A1: 1 m² 35mm
PROMATECT®-LS
Parameter Unit A1 A2 A3 A4 A5 B1 B2 B6 B7 C1 C2 C3 C4 D
GWP [kg CO2-Eq.] 1.06E+12.69E-11.26E+11.19E-12.64E+00.00E+00.00E+00.00E+00.00E+00.00E+05.71E-20.00E+02.52E-1-4.78E-1
6.30E- 1.63E- 3.19E- 7.30E- 1.53E- 1.38E- -7.42E-
ODP [kg CFC11-Eq.] 1.46E-8 0.00E+00.00E+00.00E+00.00E+00.00E+0 0.00E+0
17 12 17 10 17 15 15
AP [kg SO2-Eq.] 1.98E-2 2.30E-3 7.33E-3 9.47E-5 1.70E-30.00E+00.00E+00.00E+00.00E+00.00E+04.54E-50.00E+01.51E-3-5.01E-4
EP [kg (PO4)3--Eq.] 2.35E-3 2.80E-4 1.98E-3 1.86E-5 2.72E-40.00E+00.00E+00.00E+00.00E+00.00E+08.91E-60.00E+01.71E-4-7.49E-5
POCP [kg ethene-Eq.] 2.55E-3 1.19E-4 1.12E-3-1.20E-62.07E-40.00E+00.00E+00.00E+00.00E+00.00E+0-5.73E-70.00E+01.16E-4-5.15E-5
ADPE [kg Sb-Eq.] 1.15E-6 2.01E-8 1.67E-6 1.08E-8 1.47E-70.00E+00.00E+00.00E+00.00E+00.00E+05.15E-90.00E+02.53E-8-8.48E-8
-
ADPF [MJ] 6.82E+13.52E+02.28E+21.60E+01.55E+10.00E+00.00E+00.00E+00.00E+00.00E+07.65E-10.00E+03.42E+0
6.84E+0
GWP = Global warming potential; ODP = Depletion potential of the stratospheric ozone layer; AP = Acidification potential of land and water; EP =
Caption Eutrophication potential; POCP = Formation potential of tropospheric ozone photochemical oxidants; ADPE = Abiotic depletion potential for non-
fossil resources; ADPF = Abiotic depletion potential for fossil resources
RESULTS OF THE LCA - INDICATORS TO DESCRIBE RESOURCE USE according to EN 15804+A1: 1 m²
35mm PROMATECT®-LS
Parameter Unit A1 A2 A3 A4 A5 B1 B2 B6 B7 C1 C2 C3 C4 D
PERE [MJ] 1.91E+1 1.58E-1 1.80E+1 9.29E-2 1.59E+1 0.00E+0 0.00E+0 0.00E+0 0.00E+0 0.00E+0 4.45E-2 0.00E+0 2.63E+0 -1.91E+0
PERM [MJ] 2.34E+0 0.00E+0 1.31E+1 0.00E+0 -1.32E+1 0.00E+0 0.00E+0 0.00E+0 0.00E+0 0.00E+0 0.00E+0 0.00E+0 -2.15E+0 0.00E+0
PERT [MJ] 2.14E+1 1.58E-1 3.10E+1 9.29E-2 2.72E+0 0.00E+0 0.00E+0 0.00E+0 0.00E+0 0.00E+0 4.45E-2 0.00E+0 4.75E-1 -1.91E+0
PENRE [MJ] 7.54E+1 3.57E+0 2.31E+2 1.62E+0 1.62E+1 0.00E+0 0.00E+0 0.00E+0 0.00E+0 0.00E+0 7.76E-1 0.00E+0 3.53E+0 -8.42E+0
PENRM [MJ] 0.00E+0 0.00E+0 6.12E-2 0.00E+0 -6.12E-2 0.00E+0 0.00E+0 0.00E+0 0.00E+0 0.00E+0 0.00E+0 0.00E+0 0.00E+0 0.00E+0
PENRT [MJ] 7.54E+1 3.57E+0 2.31E+2 1.62E+0 1.61E+1 0.00E+0 0.00E+0 0.00E+0 0.00E+0 0.00E+0 7.76E-1 0.00E+0 3.53E+0 -8.42E+0
SM [kg] 2.27E+0 0.00E+0 0.00E+0 0.00E+0 1.14E-1 0.00E+0 0.00E+0 0.00E+0 0.00E+0 0.00E+0 0.00E+0 0.00E+0 0.00E+0 0.00E+0
RSF [MJ] 0.00E+0 0.00E+0 0.00E+0 0.00E+0 0.00E+0 0.00E+0 0.00E+0 0.00E+0 0.00E+0 0.00E+0 0.00E+0 0.00E+0 0.00E+0 0.00E+0
NRSF [MJ] 0.00E+0 0.00E+0 0.00E+0 0.00E+0 0.00E+0 0.00E+0 0.00E+0 0.00E+0 0.00E+0 0.00E+0 0.00E+0 0.00E+0 0.00E+0 0.00E+0
FW [m³] 1.45E-2 1.83E-4 8.31E-2 1.06E-4 8.51E-3 0.00E+0 0.00E+0 0.00E+0 0.00E+0 0.00E+0 5.09E-5 0.00E+0 8.70E-4 -1.86E-3
PERE = Use of renewable primary energy excluding renewable primary energy resources used as raw materials; PERM = Use of
renewable primary energy resources used as raw materials; PERT = Total use of renewable primary energy resources; PENRE = Use of
non-renewable primary energy excluding non-renewable primary energy resources used as raw materials; PENRM = Use of non-
Caption
renewable primary energy resources used as raw materials; PENRT = Total use of non-renewable primary energy resources; SM = Use
of secondary material; RSF = Use of renewable secondary fuels; NRSF = Use of non-renewable secondary fuels; FW = Use of net fresh
water
RESULTS OF THE LCA – WASTE CATEGORIES AND OUTPUT FLOWS according to EN 15804+A1:
1 m² 35mm PROMATECT®-LS
Parameter Unit A1 A2 A3 A4 A5 B1 B2 B6 B7 C1 C2 C3 C4 D
HWD [kg] 1.37E-3 1.49E-10 5.59E-8 8.54E-11 6.83E-5 0.00E+0 0.00E+0 0.00E+0 0.00E+0 0.00E+0 4.09E-11 0.00E+0 3.74E-10 -1.89E-9
NHWD [kg] 4.02E-1 5.11E-4 1.25E+0 2.54E-4 9.76E-1 0.00E+0 0.00E+0 0.00E+0 0.00E+0 0.00E+0 1.22E-4 0.00E+0 1.76E+1 -3.96E-3
RWD [kg] 2.40E-3 5.87E-6 1.33E-3 2.94E-6 2.07E-4 0.00E+0 0.00E+0 0.00E+0 0.00E+0 0.00E+0 1.41E-6 0.00E+0 3.69E-5 -6.14E-4
CRU [kg] 0.00E+0 0.00E+0 0.00E+0 0.00E+0 0.00E+0 0.00E+0 0.00E+0 0.00E+0 0.00E+0 0.00E+0 0.00E+0 0.00E+0 0.00E+0 0.00E+0
MFR [kg] 0.00E+0 0.00E+0 1.68E-1 0.00E+0 8.40E-3 0.00E+0 0.00E+0 0.00E+0 0.00E+0 0.00E+0 0.00E+0 0.00E+0 0.00E+0 0.00E+0
MER [kg] 0.00E+0 0.00E+0 0.00E+0 0.00E+0 0.00E+0 0.00E+0 0.00E+0 0.00E+0 0.00E+0 0.00E+0 0.00E+0 0.00E+0 0.00E+0 0.00E+0
EEE [MJ] 0.00E+0 0.00E+0 0.00E+0 0.00E+0 2.09E+0 0.00E+0 0.00E+0 0.00E+0 0.00E+0 0.00E+0 0.00E+0 0.00E+0 0.00E+0 0.00E+0
EET [MJ] 0.00E+0 0.00E+0 0.00E+0 0.00E+0 3.77E+0 0.00E+0 0.00E+0 0.00E+0 0.00E+0 0.00E+0 0.00E+0 0.00E+0 0.00E+0 0.00E+0
HWD = Hazardous waste disposed; NHWD = Non-hazardous waste disposed; RWD = Radioactive waste disposed; CRU = Components
Caption for re-use; MFR = Materials for recycling; MER = Materials for energy recovery; EEE = Exported electrical energy; EET = Exported
thermal energy
6. LCA: Interpretation
The following graph provides information on the
relative contributions of the declared modules to
various environmental impact categories.
It can be seen that the main contributions to the impact For the raw materials, very important impacts (>25 %)
categories are coming from the production stage, more are mainly coming from the lime (GWP, ODP,
specifically from the raw material and the EP,POCP, ADPF), the cement (AP), the fibres (GWP,
manufacturing. The transport of the raw materials, the AP, ADPE) and the silica sand (ADPE).
transport of the product to the building site, the waste For the manufacturing, impacts are mainly coming
treatment of the packaging and the end-of-life modules from the energy required for the production process for
only contribute to a minor extent. heating the reactors to form the calcium silicate and for
drying the boards.
7. Requisite evidence
"<" means that the measurements were below the
quantification limit)
7.1 Radioactivity measurements Name Value Unit
Radioactivity measurements on PROMATECT®-LS Total VOC after 28d (C6-C16)
7.1 µg/m³
confirmed that it did not contain other gamma emitters Limit : 1000
than those originating from natural radiation sources. R after 28d (c/NIK) 0.017 -
The measured radioactivity levels do not exceed the Sum of VVOC after 28d (<n-C6) <5 µg/m³
activity concentration indices as specified by Article 3 Sum of SVOC after 28d (>n-C16)
<5 µg/m³
(Radiation Protection 112) for building products Limit : 100
following the Council Sum of cancerogenic
<1 µg/m³
Directive 96/29. Activity concentration index ≤ 2. Limit : 1
Date: 2 December 2011 Formaldehyd
Measuring agency: SCK.CEN Laboratory for Limit : 120 <5 µg/m³
Gammaspectrometry, Mol, Belgium Acetaldehyd <5 µg/m³
Protocol: Activity concentration index (ACI)
Date: 30 September 2008
Measuring agency: Eurofins Product Testing A/S,
Galten, Denmark
7.2 VOC emissions
Report number: 765392F
PROMATECT®-LS complies with the requirements of
DIBt /DIBt-communication 4/2004/ in combination with
the NIK values from AgBB (March 2008) for use in the
indoor environment. (values in the table below having
8. References
8 Environmental Product Declaration Etex Building Performance NV – PROMATECT®-LS
Standards Nachhaltiges Bauen (BNB)" Sustainable Building
Information Portal by the Federal Ministry of Transport,
EN 826 Building and Urban Affairs (Bundesinstitut für Bau-
EN 826: 1996: Thermal insulating products for building ,Stadt-und Raumforschung, BBSR).
applications - Determination of compression behaviour (https://www.nachhaltigesbauen.de/baustoff-
undgebaeudedaten/
EN 1607 nutzungsdauern-von-bauteilen.html)
EN 1607: 1996: Thermal insulating products for
building applications - Determination of tensile strength Candidate list
perpendicular to faces Candidate List of substances of very high concern for
Authorisation, published on ECHA website, latest
EN 1608 version 19.01.2021. (https://echa.europa.eu/candidate-
EN 1608: 1996: Thermal insulating products for list-table)
building applications - Determination of tensile strength
parallel to faces CPR
Construction Products Regulation, Regulation (EU) No
EN 12467 305/2011 of the European Parliament and of the
EN 12467: 2004: Fibre-cement flat sheets - Product Council of 9 March 2011 laying down harmonized
specification and test methods conditions for the marketing of construction products
and repealing Council Directive 89/106/ EEC Text with
EN 12667 EEA relevance.
EN 12667: 2001: Thermal performance of building
materials and products- Determination of thermal DIBt-communication 4/2004
resistance by means of guarded hot plate and heat DIBt (Deutsches Institut für Bautechnik) approval
flow meter methods. Products of high and medium guidelines for the health-related evaluation of indoor
thermal resistance. construction products-2004
EN 13501-1 Directive 96/29
EN 13501-1:2018, Fire classification of construction Council Directive 96/29/Euratom of 13 May 1996 laying
products and building elements - Part 1: Classification down basic safety standards for the protection of the
using data from reaction to fire tests. health of workers and the general public against the
dangers arising from ionising radiation
EN 15804
EN 15804:2012+A2:2019, Sustainability of European List of Waste
construction works — Environmental Product 2014/955/EU: Commission Decision of 18 December
Declarations — Core rules for the product category of 2014 amending Decision 2000/532/EC on the list of
construction products. waste pursuant to Directive 2008/98/EC of the
European Parliament and of the Council.
ISO 9001 (http://data.europa.eu/eli/dec/2014/955/oj)
UNI EN ISO 9001:2015 September 2015, Quality
management systems - Requirements ETA 11/0039
European technical approval of PROMATECT®-LS fire
ISO 12572 protective board
DIN EN ISO 12572:2001, Hygrothermal performance
of building materials and products - Determination of Eurofins Product Testing A/S
water vapour transmission properties - Cup method Eurofins Product Testing A/S, Smedeskovvej 38, 8464
Galten, Denmark. Report number: 765392F; 2008.
ISO 14001
UNI EN ISO 14001:2015, Environmental management GaBi
systems - Requirements with guidance for use. GaBi Software System and Database for Life Cycle
Engineering, 1992-2021, Sphera Solutions GmbH,
ISO 14025 Leinfelden-Echterdingen, with acknowledgement of
DIN EN ISO 14025:2011-10, Environmental labels and LBP University of Stuttgart, program version GaBi 10;
declarations — Type III environmental declarations — database version 2021.1.
Principles and procedures.
GaBi documentation
ISO 45001 GaBi dataset documentation for the software system
ISO 45001:2018, Occupational health and safety and databases, LBP, University of Stuttgart and
management systems — Requirements with guidance Sphera Solutions GmbH, Leinfelden-Echterdingen,
for use 2021.
(http://www.gabi-software.com/support/gabi/gabi-
Further References database-2021-lci-documentation/)
AgBB IBU 2021
Ausschuss zur gesundheitlichen Bewertung von Institut Bauen und Umwelt e.V.: General Programme
Bauprodukten, AgBB (eng. German Committee for Instructions for the Preparation of EPDs at the Institut
health-related evaluation of building products. Bauen und Umwelt e.V. Version 2.0, Berlin: Institut
Bauen und Umwelt e.V., 2021.
BBSR (http://www.ibu-epd)
BBSR table "Service lives of components for life cycle
assessment according to Bewertungssystem Ordinance on Biocide Products
9 Environmental Product Declaration Etex Building Performance NV – PROMATECT®-LS
Regulation (EU) No 528/2012 of the European Regulation (EU) No 1907/2006 of the European
Parliament and of the Council of 22 May 2012 Parliament and of the Council of 18 December 2006
concerning the making available on the market and concerning the Registration, Evaluation, Authorisation
use of biocidal products. and Restriction of Chemicals (REACH), establishing a
European Chemicals Agency, amending Directive
PCR Part A 1999/45/EC and repealing Council Regulation (EEC)
PCR Part A: Calculation rules for the Life Cycle No 793/93 and Commission
Assessment and Requirements on the Background Regulation (EC) No 1488/94 as well as Council
Report according to EN 15 804+A2:2019, Version 1.0, Directive 76/769/EEC and Commission Directives
Institut Bauen und Umwelt e.V., 2020. 91/155/EEC, 93/67/EEC, 93/105/EC and 2000/21/EC.
PCR Part B SCK CEN Laboratory
Product Category Rules for Building Products, Part B: Belgian Nuclear Research Centre in Mol.
Requirements on the EPD for Calcium silicate
insulating materials, version 1.6, 2017 www.bau-
umwelt.de
REACH Regulation
10 Environmental Product Declaration Etex Building Performance NV – PROMATECT®-LS
Publisher
Institut Bauen und Umwelt e.V. Tel +49 (0)30 3087748- 0
Panoramastr. 1 Fax +49 (0)30 3087748- 29
10178 Berlin Mail info@ibu-epd.com
Germany Web www.ibu-epd.com
Programme holder
Institut Bauen und Umwelt e.V. Tel +49 (0)30 - 3087748- 0
Panoramastr 1 Fax +49 (0)30 – 3087748 - 29
10178 Berlin Mail info@ibu-epd.com
Germany Web www.ibu-epd.com
Author of the Life Cycle
Assessment Tel +32 (0)15 71 82 83
Peggy Van De Velde Fax +32 (0)15 71 82 29
Bormstraat 24 Mail
2830 Tisselt peggy.vandevelde@etexgroup.c
Belgium om
Web www.etexgroup.com
Owner of the Declaration
Etex Building Performance Tel +32 2 778 12 11
International Fax +32 2 778 12 12
Rue Marcel Demonque 500 r Mail info@etexgroup.com
84915 Avignon Cedex 9 Web http://www.etexgroup.com
France
