ENVIRONMENTAL PRODUCT DECLARATION
as per ISO 14025 and EN 15804+A2
Owner of the Declaration Etex Building Performance International
Programme holder Institut Bauen und Umwelt e.V. (IBU)
Publisher Institut Bauen und Umwelt e.V. (IBU)
Declaration number EPD-PMT-20210153-IBC2-EN
Issue date 30.11.2021
Valid to 05.09.2026
PROMATECT®-L / PROMATECT®-L500 /
PROMATECT®-AD / VERMICULUX-S
Medium density calcium silicate fire protective boards
Promat
www.ibu-epd.com | https://epd-online.com
Umwelt Produktdeklaration Name des Herstellers – Name des Produkts
1. General Information
Etex Building Performance NV PROMATECT®-L /
PROMATECT®-L500/
PROMATECT®-AD/
VERMICULUX-S
Programme holder Owner of the declaration
IBU – Institut Bauen und Umwelt e.V. Etex Building Performance International
Panoramastr. 1 500 Rue Marcel Demonque
10178 Berlin F-84915 Avignon
Germany France
Declaration number Declared product / declared unit
EPD-PMT-20210153-IBC2-EN The functional unit is 1 m² of PROMATECT®-L/-L500/-
AD and VERMICULUX-S with a thickness of 30 mm.
This declaration is based on the product Scope:
category rules: The life cycle assessment is based on production data
Calcium silicate insulating materials, 11.2017 of PROMATECT®-L/-L500/-AD and VERMICULUX-
(PCR checked and approved by the SVR) S of the year 2019 at the production site Tisselt,
Belgium.
Issue date
30.11.2021 The owner of the declaration shall be liable for the
underlying information and evidence; the IBU shall not
be liable with respect to manufacturer information, life
Valid to
cycle assessment data and evidences.
05.09.2026
The EPD was created according to the specifications
of EN 15804+A2. In the following, the standard will be
simplified as EN 15804.
Verification
The standard EN 15804 serves as the core PCR
Independent verification of the declaration and data
according to ISO 14025:2010
Dipl. Ing. Hans Peters internally x externally
(chairman of Institut Bauen und Umwelt e.V.)
Dr. Alexander Röder Vito D'Incognito
(Managing Director Institut Bauen und Umwelt e.V.)) (Independent verifier)
2. Product
2.1 Product description/Product definition  ETA 08/0130_2018-06-25_PROMATECT®-
PROMATECT®-L/-L500/-AD and VERMICULUX-S are AD;
lightweight, non-combustible, fire-resisting calcium
 ETA 19/0434_2020-02-04_VERMICULUX-S
silicate boards, not sensitive to moisture.
All boards are manufactured in the same plant, using
the same production technology and similar raw and the CE-marking. For the application and use the
materials though in different quantities. respective national provisions apply.
The functional unit refers to a weighted average
product based on the ratio of tons produced of the 2.2 Application
products in the reference year 2019. PROMATECT®-L/-L500/-AD and VERMICULUX-S are
primarily used in interior building applications where
For the placing of the product on the market in the normal to high levels of fire resistance are required.
European Union/European Free Trade Association The boards are intended to protect elements or to be
/EU/EFTA) (with the exception of Switzerland) the used in technical services assemblies.
Regulation (EU) No. 305/2011 (CPR) applies. The Main application areas are the fire protection of ducts
products need a declaration of performance taking into such as cable, ventilation and smoke extraction ducts,
consideration fire protection to structural steel and fire protection of
 ETA 07/0296_2018-03-25_PROMATECT®- mechanical and electrical service enclosures.
L;
 ETA 06/0218_2018-06-25_PROMATECT®-
L500
2 Environmental Product Declaration Etex Building Performance NV – PROMATECT®-L / PROMATECT®-L500 /
PROMATECT®-AD / VERMICULUX-S
2.3 Technical Data (EU) Ordinance on Biocide Products No. 528/2012):
no.
Constructional data 2.6 Manufacture
Sand, water and lime are mixed and blended in a
reactor to form calcium silicate. This is combined in a
Name Value Unit mixer with the other raw materials to form a thick
Gross density 23°C, 50%RH; slurry. The slurry is formed to a board in a filter press.
according to ETA 07/0296; ETA 400 - Boards are dried, edges are trimmed and the upper
kg/m3
06/0218; ETA 08/0130 and ETA 580 surface is sanded to the specific thickness. All material
19/0434 which is cut off or sanded away is fully recycled within
Compressive strength according to EN the process.
4.2 N/mm2
826
Tensile strength (perpendicular)
0.057 N/mm2
according to EN 1607
Flexural strength according to EN
1.7 N/mm2
12467
Thermal conductivity according to EN
0.09 W/(mK)
12667
Water vapour diffusion resistance
3.2 -
factor according to EN 12572
Tensile strength (parallel) according to
445 kPa
EN 1608
Values are guidance values and do not reflect a
statistical evaluation or guaranteed value.
Performance data of the product in accordance with
the declaration of performance with respect to its
essential characteristics according to ETA 07/0296; The quality management system of the company and
ETA 06/0218; ETA 08/0130 and ETA 19/0434. the production facility are certified according to ISO
9001.
2.4 Delivery status
Fire protective calcium silicate boards are delivered in 2.7 Environment and health during
various formats and thicknesses: manufacturing
Promat commits to a clean, healthy and safe working
 PROMATECT®-L: available in 1200 x 2500 environment for every person working in and for the
mm in 15,20,25,30,40 and 50 mm and company.
available in 1200 x 30000 mm in 20,25,30,40 The company and the manufacturing site have an
environment, health and safety management system
and 50 mm.
which is ISO 14001 and ISO 45001 certified. The
 PROMATECT®-L500: available in 1200 x
manufacturing plant adheres to the Belgium
2500 mm in 20,25,30,35,40,50,52 and 60 mm
environmental and health and safety regulations.
and available in 1220 x 2440 in 50 mm.
 PROMATECT®-AD: available in 1200 x 2500 2.8 Product processing/Installation
mm in 20,25,30,35,40,50,52 and 60 mm. The fire protective board is cut and machined using
conventional woodworking equipment.
 VERMICULUX-S: available in 1200 x 2500
Fixing the boards will require appropriate means,
mm in 20,25,30,35,40,50,52 and 60 mm and
which will depend upon the application and bearing
available in 1220 x 2440 in 50 mm. structure. Boards can be installed using screws or
glues.
Industrial and environmental protection are assured
2.5 Base materials/Ancillary materials through training and coaching staff on safety and
Main raw materials used (in weight percentages): environmental impacts. Dust levels are kept low by
- sand: 25-45% performing dust extraction. Noise is reduced by noise
- lime: 25-45% insulation on the machines and ear protection is
- cement: <25% provided for persons entering the production area.
- fibres: <6% Regular measurements on noise and dust are
Reaction is performed in an aqueous suspension. performed and show conformity to the permitted
levels.
This article contains substances listed in the candidate All national, local and other applicable safety
list (date: 19.01.2021) exceeding 0.1 percentage by regulations are complied with.
mass: no.
This article contains other carcinogenic, mutagenic, 2.9 Packaging
reprotoxic (CMR) substances in categories 1A or 1B All fire protection boards are packed onto wooden
which are not on the candidate list, exceeding 0.1 pallets, wrapped with polyester strapping tape and
percentage by mass: no. strengthened with cardboard corners.
Biocide products were added to this construction
product or it has been treated with biocide products
(this then concerns a treated product as defined by the
3 Environmental Product Declaration Etex Building Performance NV – PROMATECT®-L / PROMATECT®-L500 /
PROMATECT®-AD / VERMICULUX-S
2.10 Condition of use
PROMATECT®-L/-L500/-AD and VERMICULUX-S Mechanical destruction
boards are resistant to the effects of moisture and will In order to prevent any reduction of fire performance
not physically deteriorate when used in damp or humid following unforeseeable mechanical destruction, all
conditions. Performance characteristics are not damage of the components needs to be repaired using
degraded by age or moisture. Boards do not materials specified by the ETA 07/0296; ETA 06/0218;
encourage mould growth and are resistant to attacks ETA 08/0130 or ETA 19/0434.
by insects or vermin. Besides the need for repair, the destruction will not
have any significant environmental impact.
2.11 Environment and health during use
PROMATECT®-L/-L500/-AD and VERMICULUX-S 2.14 Re-use phase
boards are chemically inert. When the products are Several possibilities exist for the boards after the end-
used as designed, the current state of knowledge of-life of the application in which they were used.
indicates that there is no risk involved for the If the boards are removed non-destructively by
environment or health. releasing the screws, the undamaged product can be
re-used in accordance with the original purpose.
2.12 Reference service life If not contaminated with other building construction
The service life according to the "Bundesinstitut für material, the boards also allow being recycled by the
Bau-, Stadt- und Raumforschung" (BBSR) table is manufacturer.
indicated to be ≥ 50 years. Furthermore, the products referred to could be used as
The reference service life (RSL) is therefore estimated filler and bulk material in civil engineering, as an
to be 50 years. This RSL corresponds to the period absorber in cat litter or be recycled in the cement
after which a building renovation is usually needed, industry.
independently of the actual lifetime of the product For this EPD, a conservative worst-case scenario was
(which can be longer than 50 years). chosen at the end-of-life stage and the product was
sent for 100% to landfill.
2.15 Disposal
2.13 Extraordinary effects Within the production process, generated waste is re-
used within the process.
Fire When after end-of-life reusing or recycling the boards
The PROMATECT®-L/-L500/-AD and VERMICULUX- as described in the previous paragraph is not practical,
S boards have a reaction to fire classification A1 or the boards can be disposed to landfill without pre-
non-combustible according to EN13501-1. treatment thanks to the largely mineral ingredients
resulting in an inert matrix, The waste code in
Fire protection accordance with the European List of Waste is
Name Value 170904.
Building material class A1
Burning droplets - 2.16 Further information
Smoke gas development - Further information is available on the following web
site :
Water https://www.promat.com
All ingredients are firmly bound in the matrix. The
boards are insensitive to moisture and no ingredients
which could be hazardous to water are washed out in
the event of extraordinary effects by water.
3. LCA: Calculation rules
3.1 Declared Unit Adjustment factor to 1m² 15 mm
The declared unit is 1 m² of PROMATECT®-L/-L500/- (multiply results by this factor to 0.50 -
AD and VERMICULUX-S with a thickness of 30mm. obtain the results for 1m² 15 mm)
The results for other thicknesses can be obtained by Adjustment factor to 1m² 20 mm
multiplying the presented results by the corresponding (multiply results by this factor to 0.67 -
adjustment factor as included in the table. obtain the results for 1m² 20 mm)
This unit refers to a weighted average product based Adjustment factor to 1m² 25 mm
on the ratio of tons produced of all products in the (multiply results by this factor to 0.83 -
reference year 2019. obtain the results for 1m² 25 mm)
Adjustment factor to 1m² 35 mm
Declared unit (multiply results by this factor to 1.17 -
Name Value Unit obtain the results for 1m² 35 mm)
Gross density 490 kg/m3 Adjustment factor to 1m² 40 mm
Grammage 14.7 kg/m2 (multiply results by this factor to 1.33 -
Declared unit 1.00 m² obtain the results for 1m² 40 mm)
Conversion factor to 1 kg (divide Adjustment factor to 1m² 50 mm
results by this factor to obtain the 14.7 - (multiply results by this factor to 1.67 -
results for 1 kg) obtain the results for 1m² 50 mm)
Adjustment factor to 1 ton Adjustment factor to 1m² 52 mm
1.73 -
(multiply results by this factor to 68.03 - (multiply results by this factor to
obtain the results for 1ton)
4 Environmental Product Declaration Etex Building Performance NV – PROMATECT®-L / PROMATECT®-L500 /
PROMATECT®-AD / VERMICULUX-S
obtain the results for 1m² 52 mm) Assumptions and approximations were applied in case
Adjustment factor to 1m² 60 mm of a lack of representative data.
(multiply results by this factor to 2.00 - There were no data records in the GaBi database
obtain the results for 1m² 60 mm)) available for the wooden pallets, they were
approximated using the "Solid construction timber"
All boards declared in this EPD are produced at the dataset.
Etex Building Performance production site in Tisselt The waste water treatment of process water was
using the same production technology and similar raw approximated by datasets of municipal waste water
materials though in different quantities. The calculation treatment, which will result in an overestimation of
of the weighted average recipe and grammage is impacts.
based on the ratio of tons produced of All assumptions and approximations were documented
PROMATECT®-L/-L500/-AD and VERMICULUX-S in precisely.
2019.
3.4 Cut-off criteria
3.2 System boundary In the assessment, all utilised raw material, thermal
Type of the EPD: cradle to grave. energy and electric power were considered using
The following life cycle stages and modules are GaBi datasets. Only the transport of packaging,
included: production waste to recycling/disposal and of
installation loss waste to recycling was cut-off in this
Production stage (A1-A3): study.
 pre-chains of the raw materials and their Production of capital equipment, facilities and
infrastructure required for the manufacture are outside
transportation to the manufacturing site
the scope of the study and thus were not included.
 energy consumption during production
 recycling and disposal of production wastes 3.5 Background data
 production of packaging Background data were sourced from GaBi 10 database
version 2021.
3.6 Data quality
Construction stage (A4-A5):
This study is mainly based on primary data collected
 transportation of product to the construction
directly from the manufacturing site and therefore data
site
quality can be assumed to be very good.
 disposal of installation wastes The last update of the GaBi database used for
 incineration of packaging materials (potential the background data was February 2021.
benefits from energy substitution within the
3.7 Period under review
incineration process are declared in module
Data for the entire production period of 2019 were
D)
collected and used for this EPD.
3.8 Allocation
Use stage (B1-B7): Allocation in background data
 efforts for the use of the product, Specific information on allocation within the
maintenance and operational efforts background data is given in the GaBi documentation.
Allocation in foreground data
 modules B3, B4, B5 are declared as MNR
The production process does not deliver any co-
(module not relevant) according to the IBU
products. In modules A1 to A3, specific raw material
requirement. These modules are defined on and transport data were available, energy, waste and
building level in general water could not be directly allocated to the product and
were allocated via the production volume of the
specific products.
Allocation for waste materials
End-of-life stage (C1-C4):
The environmental burden of the incineration of
 transport to disposal of the material
packaging in the construction process stage is
 landfill end-of-life scenario was considered
assigned to the system (A5); resulting credits for
thermal and electrical energy are declared in module
D.
Loads and benefits beyond system boundary (D):
 loads and benefits from the recycling of
3.9 Comparability
production waste and incineration of
Basically, a comparison or an evaluation of EPD data
packaging waste
is only possible if all the data sets to be compared
were created according to EN 15804 and the building
context, respectively the product-specific
3.3 Estimates and assumptions characteristics of performance, are taken into account.
Most of the input and output influences of the Life
Cycle Inventory Analysis could be depicted using GaBi database version 2021.1 serves as a
corresponding data from the GaBi database. background database for the calculation of the life
cycle assessment.
5 Environmental Product Declaration Etex Building Performance NV – PROMATECT®-L / PROMATECT®-L500 /
PROMATECT®-AD / VERMICULUX-S
4. LCA: Scenarios and additional technical information
Characteristic product properties Auxiliary - kg
Information on biogenic Carbon Other resources - kg
The biogenic carbon content quantifies the amount of Electricity consumption - kWh
biogenic carbon in the construction product leaving the Other energy carriers - MJ
factory gate. It is declared separately for the product Material loss - kg
and the accompanying packaging.
Replacement (B4) / Refurbishment (B5)
Information on describing the biogenic Carbon
Name Value Unit
Content at factory gate Number/
Name Value Unit Replacement cycle - RSL
Biogenic Carbon Content in product 0.08 kg C
Electricity consumption - kWh
Biogenic Carbon Content in
0.29 kg C Litres of fuel - l/100km
accompanying packaging
Replacement of worn parts - kg
Reference service life
Name Value Unit
Transport to the building site (A4)
Reference service life - a
For the transport from the factory gate to the building
Life Span (according to BBSR) >=50 a
site, an average distance of 100km was assumed. This
Life Span according to the
distance can be assumed to be representative of - a
manufacturer
deliveries within Belgium.
Declared product properties (at the
- -
gate) and finishes
Name Value Unit
Design application parameters (if
Litres of fuel 0.031 l/100km
instructed by the manufacturer),
Transport distance 100 km
including the references to the - -
Capacity utilisation (including empty
61 % appropriate practices and application
runs)
codes
Gross density of products transported 490 kg/m3
An assumed quality of work, when
installed in accordance with the - -
manufacturer’s instructions
Outdoor environment, (for outdoor
Installation into the building (A5)
applications), e.g. weathering,
Only waste treatment of installation loss and packaging
pollutants, UV and wind exposure, - -
is considered in this module.
building orientation, shading,
Installation into the building (A5)
temperature
Name Value Unit
Indoor environment (for indoor
Material loss 0.74 kg
applications), e.g. temperature, - -
VOC in the air 0 kg
moisture, chemical exposure
Usage conditions, e.g. frequency of
- -
use, mechanical exposure
Use or application of the installed product (B1) see
Maintenance e.g. required frequency,
section 2.12 "Use"
type and quality and replacement of - -
No efforts and releases of substances occur during
components
the normal (i.e. anticipated) use phase.
Name Value Unit
Operational energy use (B6) and Operational water
use (B7)
Maintenance (B2)
No efforts occur in modules B6 and B7.
No efforts occur during maintenance.
Name Value Unit
Name Value Unit
Water consumption 0 m3
Number/
Maintenance cycle 0 Electricity consumption 0 kWh
RSL
Water consumption 0 m3 Other energy carriers 0 MJ
Equipment output 0 kW
Auxiliary 0 kg
Other resources 0 kg
End-of-life (C1-C4)
Electricity consumption 0 kWh
A conservative approach was used in this study.
Other energy carriers 0 MJ
Although after end-of-life, scenarios where the
Material loss 0 kg
boards are re-used or recycled are realistic, a
scenario with 100% landfill was used.
Repair (B3)
Name Value Unit
Name Value Unit
Landfilling 14.7 kg
Information on the repair process - -
Information on the inspection process - -
Re-use, recovery and/or recycling potentials (D),
Number/
Repair cycle - relevant scenario information
RSL
Although re-use and recycling of the PROMATECT®-
Water consumption - m3
L/-L500/-AD and VERMICULUX-S is possible, this is
6 Environmental Product Declaration Etex Building Performance NV – PROMATECT®-L / PROMATECT®-L500 /
PROMATECT®-AD / VERMICULUX-S
not yet a widely established practice. Therefore, no
possible benefits of recycling or re-use of the boards
were taken into account in this study. In module D,
only the benefits from recycling of production waste
and incineration of waste packaging were taken into
account.
Name Value Unit
Exported electrical energy 1.8 MJ
Exported thermal energy 3.2 MJ
7 Environmental Product Declaration Etex Building Performance NV – PROMATECT®-L / PROMATECT®-L500 /
PROMATECT®-AD / VERMICULUX-S
5. LCA: Results
The following tables depict the results of the indicators for the Life Cycle Assessment, use of resources and waste
with reference to 1 m² of PROMATECT®-L/L500/-AD and VERMICULUX-S with a thickness of 30 mm.
Disclaimer:
EP-freshwater: This indicator has been calculated as “kg P eq” as required in the characterization model
(EUTREND model, Struijs et al., 2009b, as implemented in ReCiPe;
http://eplca.jrc.ec.europa.eu/LCDN/developerEF.xhtml).
DESCRIPTION OF THE SYSTEM BOUNDARY (X = INCLUDED IN LCA; ND = MODULE OR INDICATOR NOT
DECLARED; MNR = MODULE NOT RELEVANT)
BENEFITS AND
CONSTRUCTI LOADS
PRODUCT STAGE ON PROCESS USE STAGE END OF LIFE STAGE BEYOND THE
STAGE SYSTEM
BOUNDARIES
8 Environmental Product Declaration Etex Building Performance NV – PROMATECT®-L / PROMATECT®-L500 /
PROMATECT®-AD / VERMICULUX-S
lairetam
waR
ylppus tropsnarT
gnirutcafunaM
eht
morf
tropsnarT
etis
eht
ot
etag
ylbmessA esU
ecnanetniaM
riapeR
tnemecalpeR tnemhsibrufeR
ygrene
lanoitarepO esu
retaw
lanoitarepO esu
noitcurtsnoc-eD
noitilomed tropsnarT
gnissecorp
etsaW
lasopsiD -esueR -yrevoceR -gnilcyceR laitnetop
A1 A2 A3 A4 A5 B1 B2 B3 B4 B5 B6 B7 C1 C2 C3 C4 D
X X X X X X X MNR MNR MNR X X X X X X X
RESULTS OF THE LCA - ENVIRONMENTAL IMPACT according to EN 15804+A2: 1 m² 30mm
PROMATECT®-L/-L500/-AD and VERMICULUX S
Core Indicator Unit A1 A2 A3 A4 A5 B1 B2 B6 B7 C1 C2 C3 C4 D
GWP-total [kg CO2-Eq.] 9.59E+01.17E-11.10E+11.02E-12.28E+00.00E+00.00E+00.00E+00.00E+00.00E+09.79E-20.00E+02.16E-1-4.14E-1
GWP-fossil [kg CO2-Eq.] 9.78E+01.16E-11.20E+11.02E-11.14E+00.00E+00.00E+00.00E+00.00E+00.00E+09.72E-20.00E+02.22E-1-4.12E-1
GWP-biogenic [kg CO2-Eq.] -1.98E-1-3.12E-6-9.96E-1-1.21E-41.14E+00.00E+00.00E+00.00E+00.00E+00.00E+0-1.16E-40.00E+0-6.46E-3-2.04E-3
GWP-luluc [kg CO2-Eq.] 4.79E-3 5.10E-4 1.57E-3 8.29E-4 4.30E-40.00E+00.00E+00.00E+00.00E+00.00E+07.94E-40.00E+06.53E-4-2.88E-4
1.78E- 1.04E- 2.00E- 4.33E- 1.92E- 8.63E- -4.72E-
ODP [kg CFC11-Eq.] 8.65E-9 0.00E+00.00E+00.00E+00.00E+00.00E+0 0.00E+0
17 12 17 10 17 16 15
AP [mol H+-Eq.] 1.94E-2 2.12E-3 8.79E-3 1.08E-4 1.79E-30.00E+00.00E+00.00E+00.00E+00.00E+01.03E-40.00E+01.58E-3-5.43E-4
EP-freshwater [kg PO4-Eq.] 1.02E-4 1.97E-7 5.63E-5 3.01E-7 7.98E-60.00E+00.00E+00.00E+00.00E+00.00E+02.89E-70.00E+03.73E-7-5.44E-7
EP-marine [kg N-Eq.] 4.99E-3 5.82E-4 3.97E-3 3.44E-5 5.63E-40.00E+00.00E+00.00E+00.00E+00.00E+03.30E-50.00E+04.11E-4-1.55E-4
EP-terrestrial [mol N-Eq.] 5.41E-2 6.39E-3 4.16E-2 4.09E-4 6.25E-30.00E+00.00E+00.00E+00.00E+00.00E+03.92E-40.00E+04.52E-3-1.66E-3
POCP [kg NMVOC-Eq.]1.65E-2 1.63E-3 1.11E-2 9.37E-5 1.70E-30.00E+00.00E+00.00E+00.00E+00.00E+08.96E-50.00E+01.25E-3-4.36E-4
ADPE [kg Sb-Eq.] 1.00E-6 7.14E-9 1.43E-6 8.99E-9 1.26E-70.00E+00.00E+00.00E+00.00E+00.00E+08.61E-90.00E+02.10E-8-6.86E-8
-
ADPF [MJ] 6.51E+11.48E+01.98E+21.35E+01.37E+10.00E+00.00E+00.00E+00.00E+00.00E+01.29E+00.00E+02.95E+0
7.14E+0
[m³ world-Eq
WDP 4.02E-1 6.61E-42.84E+09.42E-4 2.92E-10.00E+00.00E+00.00E+00.00E+00.00E+09.01E-40.00E+02.39E-2-3.16E-2
deprived]
GWP = Global warming potential; ODP = Depletion potential of the stratospheric ozone layer; AP = Acidification potential of land and water; EP =
Caption Eutrophication potential; POCP = Formation potential of tropospheric ozone photochemical oxidants; ADPE = Abiotic depletion potential for non-
fossil resources; ADPF = Abiotic depletion potential for fossil resources; WDP = Water (user) deprivation potential
RESULTS OF THE LCA - INDICATORS TO DESCRIBE RESOURCE USE according to EN 15804+A2: 1 m²
30mm PROMATECT®-L/-L500/-AD and VERMICULUX S
Indicator Unit A1 A2 A3 A4 A5 B1 B2 B6 B7 C1 C2 C3 C4 D
PERE [MJ] 1.72E+1 5.00E-2 1.54E+1 7.78E-2 1.35E+1 0.00E+0 0.00E+0 0.00E+0 0.00E+0 0.00E+0 7.44E-2 0.00E+0 2.65E+0 -1.62E+0
PERM [MJ] 3.06E+0 0.00E+0 1.10E+1 0.00E+0 -1.11E+1 0.00E+0 0.00E+0 0.00E+0 0.00E+0 0.00E+0 0.00E+0 0.00E+0 -2.25E+0 0.00E+0
PERT [MJ] 2.03E+1 5.00E-2 2.64E+1 7.78E-2 2.41E+0 0.00E+0 0.00E+0 0.00E+0 0.00E+0 0.00E+0 7.44E-2 0.00E+0 3.97E-1 -1.62E+0
PENRE [MJ] 6.51E+1 1.49E+0 1.98E+2 1.36E+0 1.38E+1 0.00E+0 0.00E+0 0.00E+0 0.00E+0 0.00E+0 1.30E+0 0.00E+0 2.95E+0 -7.14E+0
PENRM [MJ] 0.00E+0 0.00E+0 9.74E-2 0.00E+0 -9.74E-2 0.00E+0 0.00E+0 0.00E+0 0.00E+0 0.00E+0 0.00E+0 0.00E+0 0.00E+0 0.00E+0
PENRT [MJ] 6.51E+1 1.49E+0 1.98E+2 1.36E+0 1.37E+1 0.00E+0 0.00E+0 0.00E+0 0.00E+0 0.00E+0 1.30E+0 0.00E+0 2.95E+0 -7.14E+0
SM [kg] 1.93E+0 0.00E+0 0.00E+0 0.00E+0 9.64E-2 0.00E+0 0.00E+0 0.00E+0 0.00E+0 0.00E+0 0.00E+0 0.00E+0 0.00E+0 0.00E+0
RSF [MJ] 0.00E+0 0.00E+0 0.00E+0 0.00E+0 0.00E+0 0.00E+0 0.00E+0 0.00E+0 0.00E+0 0.00E+0 0.00E+0 0.00E+0 0.00E+0 0.00E+0
NRSF [MJ] 0.00E+0 0.00E+0 0.00E+0 0.00E+0 0.00E+0 0.00E+0 0.00E+0 0.00E+0 0.00E+0 0.00E+0 0.00E+0 0.00E+0 0.00E+0 0.00E+0
FW [m³] 1.37E-2 5.83E-5 7.12E-2 8.91E-5 7.32E-3 0.00E+0 0.00E+0 0.00E+0 0.00E+0 0.00E+0 8.52E-5 0.00E+0 7.28E-4 -1.58E-3
PERE = Use of renewable primary energy excluding renewable primary energy resources used as raw materials; PERM = Use of
renewable primary energy resources used as raw materials; PERT = Total use of renewable primary energy resources; PENRE = Use of
non-renewable primary energy excluding non-renewable primary energy resources used as raw materials; PENRM = Use of non-
Caption
renewable primary energy resources used as raw materials; PENRT = Total use of non-renewable primary energy resources; SM = Use
of secondary material; RSF = Use of renewable secondary fuels; NRSF = Use of non-renewable secondary fuels; FW = Use of net fresh
water
RESULTS OF THE LCA – WASTE CATEGORIES AND OUTPUT FLOWS according to EN 15804+A2:
1 m² 30mm PROMATECT®-L/-L500/-AD and VERMICULUX S
Indicator Unit A1 A2 A3 A4 A5 B1 B2 B6 B7 C1 C2 C3 C4 D
HWD [kg] 1.12E-3 4.89E-11 4.76E-8 7.15E-11 5.60E-5 0.00E+0 0.00E+0 0.00E+0 0.00E+0 0.00E+0 6.84E-11 0.00E+0 3.13E-10 -1.61E-9
NHWD [kg] 3.50E-1 1.96E-4 1.07E+0 2.13E-4 8.19E-1 0.00E+0 0.00E+0 0.00E+0 0.00E+0 0.00E+0 2.04E-4 0.00E+0 1.47E+1 -3.36E-3
RWD [kg] 2.33E-3 2.24E-6 1.14E-3 2.46E-6 1.90E-4 0.00E+0 0.00E+0 0.00E+0 0.00E+0 0.00E+0 2.35E-6 0.00E+0 3.09E-5 -5.21E-4
CRU [kg] 0.00E+0 0.00E+0 0.00E+0 0.00E+0 0.00E+0 0.00E+0 0.00E+0 0.00E+0 0.00E+0 0.00E+0 0.00E+0 0.00E+0 0.00E+0 0.00E+0
MFR [kg] 0.00E+0 0.00E+0 1.44E-1 0.00E+0 7.20E-3 0.00E+0 0.00E+0 0.00E+0 0.00E+0 0.00E+0 0.00E+0 0.00E+0 0.00E+0 0.00E+0
MER [kg] 0.00E+0 0.00E+0 0.00E+0 0.00E+0 0.00E+0 0.00E+0 0.00E+0 0.00E+0 0.00E+0 0.00E+0 0.00E+0 0.00E+0 0.00E+0 0.00E+0
EEE [MJ] 0.00E+0 0.00E+0 2.11E-4 0.00E+0 1.77E+0 0.00E+0 0.00E+0 0.00E+0 0.00E+0 0.00E+0 0.00E+0 0.00E+0 0.00E+0 0.00E+0
EET [MJ] 0.00E+0 0.00E+0 4.87E-4 0.00E+0 3.20E+0 0.00E+0 0.00E+0 0.00E+0 0.00E+0 0.00E+0 0.00E+0 0.00E+0 0.00E+0 0.00E+0
HWD = Hazardous waste disposed; NHWD = Non-hazardous waste disposed; RWD = Radioactive waste disposed; CRU = Components
Caption for re-use; MFR = Materials for recycling; MER = Materials for energy recovery; EEE = Exported electrical energy; EET = Exported
thermal energy
RESULTS OF THE LCA – additional impact categories according to EN 15804+A2-optional:
1 m² 30mm PROMATECT®-L/-L500/-AD and VERMICULUX S
Indicator Unit A1 A2 A3 A4 A5 B1 B2 B6 B7 C1 C2 C3 C4 D
[Disease
PM 2.56E-7 3.68E-8 2.16E-7 7.40E-10 2.74E-8 0.00E+0 0.00E+0 0.00E+0 0.00E+0 0.00E+07.08E-100.00E+0 1.97E-8 -5.82E-9
Incidence]
[kBq U235-
IRP 3.28E-1 3.25E-4 1.33E-1 3.60E-4 2.57E-2 0.00E+0 0.00E+0 0.00E+0 0.00E+0 0.00E+0 3.44E-4 0.00E+0 3.25E-3 -8.54E-2
Eq.]
ETP-fw [CTUe] 2.81E+1 1.09E+0 1.38E+1 1.00E+0 2.40E+0 0.00E+0 0.00E+0 0.00E+0 0.00E+0 0.00E+0 9.60E-1 0.00E+0 1.68E+0-1.50E+0
-6.82E-
HTP-c [CTUh] 6.20E-9 2.13E-11 1.84E-9 2.03E-114.24E-100.00E+0 0.00E+0 0.00E+0 0.00E+0 0.00E+01.94E-110.00E+02.48E-10
11
HTP-nc [CTUh] 1.01E-7 1.08E-9 4.06E-8 1.05E-9 8.82E-9 0.00E+0 0.00E+0 0.00E+0 0.00E+0 0.00E+0 1.01E-9 0.00E+0 2.74E-8 -2.70E-9
SQP [-] 9.96E+1 2.87E-1 2.17E+2 4.65E-1 1.60E+1 0.00E+0 0.00E+0 0.00E+0 0.00E+0 0.00E+0 4.45E-1 0.00E+0 5.95E-1 -1.11E+0
PM = Potential incidence of disease due to PM emissions; IR = Potential Human exposure efficiency relative to U235; ETP-fw = Potential
Caption comparative Toxic Unit for ecosystems; HTP-c = Potential comparative Toxic Unit for humans (cancerogenic); HTP-nc = Potential
comparative Toxic Unit for humans (not cancerogenic); SQP = Potential soil quality index
Disclaimer 1 – for the indicator IRP
This impact category deals mainly with the eventual impact of low dose ionizing radiation on human health of the
nuclear fuel cycle. It does not consider effects due to possible nuclear accidents, occupational exposure nor to
radioactive waste disposal in underground facilities. Potential ionizing radiation from the soil, from radon and from
some construction materials is also not measured by this indicator.
Disclaimer 2 – for the indicators ADPE, ADPF, WDP, ETP-fw, HTP-c, HTP-nc, SQP
The results of this environmental impact indicator shall be used with care as the uncertainties on these results are
high or as there is limited experience with the indicator.
6. LCA: Interpretation
The following graph provides information on the
relative contributions of the declared modules to
various environmental impact categories.
It can be seen that the main contributions to the impact manufacturing. The transport of the raw materials, the
categories are coming from the production stage, more transport of the product to the building site, the waste
specifically from the raw material and the
9 Environmental Product Declaration Etex Building Performance NV – PROMATECT®-L / PROMATECT®-L500 /
PROMATECT®-AD / VERMICULUX-S
treatment of the packaging and the end-of-life modules heating the reactors to form the calcium silicate and for
only contribute to a minor extent. drying the boards.
For the raw materials, very important impacts (>25%) Since a weighted average product was declared, the
are mainly coming from the lime (GWP-total, GWP variance of the LCIA results of this average product
fossil, ODP, EP-freshwater, EP-marine, EP-terrestrial, was compared to the impacts of the single product. It
POCP, ADPF), the cement (EP-marine, EP-terrestrial), could be concluded that differences were relatively low
the fibres (GWP-biogenic, GWP-luluc, AP, EP-marine, and that the average environmental impacts show a
EP-terrestrial, POCP, ADPE, WDP) and the silica sand high representativity (the difference percentage
(GWP-luluc, ADPE, ADPF). between the impact of the specific product and of the
For the manufacturing, impacts are mainly coming declared average is less than 6% for all impact
from the energy required for the production process for categories except GWP-biogenic and ODP).
7. Requisite evidence
table below having "<" means that the measurements
were below the quantification limit)
7.1 Radioactivity measurements Name Value Unit
Radioactivity measurements confirm that no other Total VOC after 28d (C-C16)
13 µg/m³
gamma emitters than those originating from natural Limit : 1000
radiation sources are contained. The measured R after 28d (c/NIK) 0.032 -
radioactivity levels do not exceed the activity Sum of VVOC after 28d (<n-C6) < 5 µ g /m³
concentration indices as specified by Article 3 Sum of SVOC after 28d (>n-C16)
<5 µg/m³
(Radiation Protection 112) for building products Limit : 100
following the Council Sum of cancerogenic
<1 µg/m³
Directive 96/29. Activity concentration index ≤ 2. Limit : 1
Date: 2 December 2011 Formaldehyd
Measuring agency: SCK.CEN Laboratory for Limit : 120 <5 µg/m³
Gammaspectrometry, Mol, Belgium Acetaldehyd <5 µg/m³
Protocol: Activity concentration index (ACI)
Date: 25 September 2008
Measuring agency: Eurofins Product Testing A/S,
Galten, Denmark
7.2 VOC emissions
Report number: 765393F
VOC measurements confirmed compliance with the
requirements of DIBt DIBt-communication 4/2004 in
combination with the NIK values from AgBB (March
2008) for use in the indoor environment. (values in the
8. References
Standards EN 13501-1:2018, Fire classification of construction
products and building elements - Part 1: Classification
EN 826 using data from reaction to fire tests.
EN 826: 1996: Thermal insulating products for building
applications - Determination of compression behaviour EN 15804
EN 15804:2012+A2:2019, Sustainability of
EN 1607 construction works — Environmental Product
EN 1607: 1996: Thermal insulating products for Declarations — Core rules for the product category of
building applications - Determination of tensile strength construction products.
perpendicular to faces
ISO 9001
EN 1608 UNI EN ISO 9001:2015 September 2015, Quality
EN 1608: 1996: Thermal insulating products for management systems - Requirements
building applications - Determination of tensile strength
parallel to faces ISO 12572
DIN EN ISO 12572:2001, Hygrothermal performance
EN 12467 of building materials and products - Determination of
EN 12467: 2004: Fibre-cement flat sheets - Product water vapour transmission properties - Cup method
specification and test methods
ISO 14001
EN 12667 UNI EN ISO 14001:2015, Environmental management
EN 12667: 2001: Thermal performance of building systems - Requirements with guidance for use.
materials and products- Determination of thermal
resistance by means of guarded hot plate and heat ISO 14025
flow meter methods. Products of high and medium DIN EN ISO 14025:2011-10, Environmental labels and
thermal resistance. declarations — Type III environmental declarations —
Principles and procedures.
EN 13501-1
ISO 45001
10 Environmental Product Declaration Etex Building Performance NV – PROMATECT®-L / PROMATECT®-L500 /
PROMATECT®-AD / VERMICULUX-S
ISO 45001:2018, Occupational health and safety European technical approval of VERMICULUX-S fire
management systems — Requirements with guidance protective board
for use
Eurofins Product Testing A/S
Further References Eurofins Product Testing A/S, Smedeskovvej 38, 8464
Galten, Denmark. Report number: 765393F; 2008.
AgBB
Ausschuss zur gesundheitlichen Bewertung von GaBi
Bauprodukten, AgBB (eng. German Committee for GaBi Software System and Database for Life Cycle
health-related evaluation of building products. Engineering, 1992-2021, Sphera Solutions GmbH,
Leinfelden-Echterdingen, with acknowledgement of
BBSR LBP University of Stuttgart, program version GaBi 10;
BBSR table "Service lives of components for life cycle database version 2021.1.
assessment according to Bewertungssystem
Nachhaltiges Bauen (BNB)" Sustainable Building GaBi documentation
Information Portal by the Federal Ministry of Transport, GaBi dataset documentation for the software system
Building and Urban Affairs (Bundesinstitut für Bau- and databases, LBP, University of Stuttgart and
,Stadt-und Raumforschung, BBSR). Sphera Solutions GmbH, Leinfelden-Echterdingen,
(https://www.nachhaltigesbauen.de/baustoff- 2021.
undgebaeudedaten/ (http://www.gabi-software.com/support/gabi/gabi-
nutzungsdauern-von-bauteilen.html) database-2021-lci-documentation/)
Candidate list IBU 2016
Candidate List of substances of very high concern for Institut Bauen und Umwelt e.V.: General Programme
Authorisation, published on ECHA website, latest Instructions for the Preparation of EPDs at the Institut
version 19.01.2021. (https://echa.europa.eu/candidate- Bauen und Umwelt e.V. Version 1.1, Berlin: Institut
list-table) Bauen und Umwelt e.V., 2016.
(http://www.ibu-epd)
CPR
Construction Products Regulation, Regulation (EU) No Ordinance on Biocide Products
305/2011 of the European Parliament and of the Regulation (EU) No 528/2012 of the European
Council of 9 March 2011 laying down harmonized Parliament and of the Council of 22 May 2012
conditions for the marketing of construction products concerning the making available on the market and
and repealing Council Directive 89/106/ EEC Text with use of biocidal products.
EEA relevance.
PCR Part A
DIBt-communication 4/2004 PCR Part A: Calculation rules for the Life Cycle
DIBt (Deutsches Institut für Bautechnik) approval Assessment and Requirements on the Background
guidelines for the health-related evaluation of indoor Report according to EN 15 804+A2:2019, Version 1.0,
construction products-2004 Institut Bauen und Umwelt e.V., 2020.
Directive 96/29 PCR Part B
Council Directive 96/29/Euratom of 13 May 1996 laying Product Category Rules for Building Products, Part B:
down basic safety standards for the protection of the Requirements on the EPD for Calcium silicate
health of workers and the general public against the insulating materials, version 1.6, 2017 www.bau-
dangers arising from ionising radiation umwelt.de
European List of Waste REACH Regulation
2014/955/EU: Commission Decision of 18 December Regulation (EU) No 1907/2006 of the European
2014 amending Decision 2000/532/EC on the list of Parliament and of the Council of 18 December 2006
waste pursuant to Directive 2008/98/EC of the concerning the Registration, Evaluation, Authorisation
European Parliament and of the Council. and Restriction of Chemicals (REACH), establishing a
(http://data.europa.eu/eli/dec/2014/955/oj) European Chemicals Agency, amending Directive
1999/45/EC and repealing Council Regulation (EEC)
ETA 06/0218 No 793/93 and Commission
European technical approval of PROMATECT®-L500 Regulation (EC) No 1488/94 as well as Council
fire protective board Directive 76/769/EEC and Commission Directives
91/155/EEC, 93/67/EEC, 93/105/EC and 2000/21/EC.
ETA 07/0296
European technical approval of PROMATECT®-L fire SCK CEN Laboratory
protective board Belgian Nuclear Research Centre in Mol.
ETA 08/0130
European technical approval of PROMATECT®-AD
fire protective board
ETA 19/0434
11 Environmental Product Declaration Etex Building Performance NV – PROMATECT®-L / PROMATECT®-L500 /
PROMATECT®-AD / VERMICULUX-S
Publisher
Institut Bauen und Umwelt e.V. Tel +49 (0)30 3087748- 0
Panoramastr. 1 Fax +49 (0)30 3087748- 29
10178 Berlin Mail info@ibu-epd.com
Germany Web www.ibu-epd.com
Programme holder
Institut Bauen und Umwelt e.V. Tel +49 (0)30 - 3087748- 0
Panoramastr 1 Fax +49 (0)30 – 3087748 - 29
10178 Berlin Mail info@ibu-epd.com
Germany Web www.ibu-epd.com
Author of the Life Cycle
Assessment Tel +32 (0)15 71 82 83
Peggy Van De Velde Fax +32 (0)15 71 82 29
Bormstraat 24 Mail
2830 Tisselt peggy.vandevelde@etexgroup.c
Belgium om
Web www.etexgroup.com
Owner of the Declaration
Etex Building Performance Tel +32 2 778 12 11
International Fax +32 2 778 12 12
Rue Marcel Demonque 500 r Mail info@etexgroup.com
84915 Avignon Cedex 9 Web http://www.etexgroup.com
France
