ENVIRONMENTAL PRODUCT DECLARATION
as per ISO 14025 and EN 15804+A2
Owner of the Declaration RBS Germany GmbH
Publisher Institut Bauen und Umwelt e.V. (IBU)
Programme holder Institut Bauen und Umwelt e.V. (IBU)
Declaration number EPD-RAV-20230375-CBD1-EN
Issue date 31.10.2023
Valid to 30.10.2028
RAVATHERM™ XPS (X) extruded polystyrene foam insulation with
non-halogenated blowing agents
Ravago Building Solutions
www.ibu-epd.com | https://epd-online.com
General Information
Ravago Building Solutions RAVATHERM™ XPS (X) extruded polystyrene foam
insulation with non-halogenated blowing agents
Programme holder Owner of the declaration
IBU – Institut Bauen und Umwelt e.V. RBS Germany GmbH
Hegelplatz 1 Value Park Y51
10117 Berlin 06258 Schkopau
Germany Germany
Declaration number Declared product / declared unit
EPD-RAV-20230375-CBD1-EN The EPD applies to 1 m3 of XPS board, with an average density of 34.4
kg/m3.
RAVATHERMTM XPS (X) extruded polystyrene foam boards produced by
Ravago Building Solutions with a non-halogenated blowing agent system.
This declaration is based on the product category rules: Scope:
Insulating materials made of foam plastics, 01.08.2021 The data have been provided by the seven ISO 14001 certified factories of
(PCR checked and approved by the SVR) Ravago Building Solutions producing these products in France, Germany,
Greece, Hungary and the UK for the year 2021.
The owner of the declaration shall be liable for the underlying information
Issue date and evidence; the IBU shall not be liable with respect to manufacturer
information, life cycle assessment data and evidences.
31.10.2023
The EPD was created according to the specifications of EN 15804+A2. In
the following, the standard will be simplified as EN 15804.
Valid to
30.10.2028 Verification
The standard EN 15804 serves as the core PCR
Independent verification of the declaration and data according to ISO
14025:2011
internally X externally
Dipl.-Ing. Hans Peters
(Chairman of Institut Bauen und Umwelt e.V.)
Florian Pronold Mr Olivier Muller,
(Managing Director Institut Bauen und Umwelt e.V.) (Independent verifier)
1 Environmental Product Declaration - Ravago Building Solutions - RAVATHERM™ XPS (X) extruded polystyrene foam insulation with non-halogenated blowing agents
Product
Product description/Product definition Performance data of the product in accordance with the
RAVATHERM(TM) XPS and XPS X extruded polystyrene foams declaration of performance with respect to its essential
(XPS) are thermoplastic insulation foams produced according characteristics according to EN 13164:2012+A1:2015 - Thermal
to EN 13164 Building insulation, EN 14307 Equipment Insulation products for buildings EN 14307:2015 Thermal
insulation. Insulation products for building equipment and industrial
installations.
They are available in blue or grey board shape with a density
range from 25 to 50 kg/m3. The boards can be delivered in
various compressive strength values from 150 to 700 kPa. Base materials/Ancillary materials
To meet the need of various applications the boards are RAVATHERMTM XPS and XPS X are mostly made of
produced with different surfaces: with the extrusion skin, polystyrene (CAS 9003-53-6), blown with carbon dioxide and
planed, grooved or with thermal embossing. non-halogenated co-blowing agents altogether up to 8 % by
These XPS boards are supplied with different edge treatments weight in relation to the material input.
such as butt edge, shiplap and tongue and groove. The EPD is
related to unfaced XPS products only; Heat lamination of Basic material Mass portion
several XPS layers is included. Additional product treatment Polystyrene 89 - 93 %
is not considered. Blowing agents 5 - 8 %
For the placing on the market of the construction product in the .Carbon Dioxide 55 - 75 %
European Union/ European Free Trade Association (EU/EFTA) .Co-blowing Agents 25 - 45 %
(with the exception of Switzerland) Regulation (EU) No. Flame retardant 0 - 2 %
305/2011 (CPR) applies. The product needs a declaration of Additives (e.g. pigments) Less than 1%
performance taking into consideration the EN XPS standards
(EN 13164 Building insulation, EN 14307 Equipment Information that the product does not contain substances listed
insulation). in the Candidate List of substances of very high concern
For the application and use the respective national provisions (REACH Regulation) exceeding 0.1%: This product contains
apply. substances listed in the candidate list (date:17.01.2023)
exceeding 0.1 percentage by mass: no
Application This product contains other Carcinogenic, Mutagenic,
The variety of the performance properties of RAVATHERM XPS Reprotoxic (CMR) substances in categories 1A or 1B which are
and XPS X thermal insulation foams make them suitable for not on the candidate list, exceeding 0.1 percentage by mass:
use in a large number of applications such as: perimeter no
insulation, inverted insulation for terrace roofs, insulation of
pitched roofs, floor insulation including insulation of highly Biocide products were added to this construction product or it
loaded industrial floors, insulation of thermal bridges for exterior has been treated with biocide products (this then concerns a
walls, External Thermal Insulation Composite System (ETICS), treated product as defined by the Regulation (EU) No 528/2012
insulation of cavity walls, agricultural building ceiling insulation, on biocidal products): no
prefabricated elements e.g. building sandwich panels,
insulation for building equipment and industrial installations
(pipe sections, …). Reference service life
The durability of XPS foam is normally at least as long as the
lifetime of the building/equipment in/with which it is used or at
Technical Data least 50 years. This is explained by the superior mechanical
Acoustic properties are not relevant for XPS foams. and water resistance properties of this product.
For fire performance, these products usually achieve the fire
classification Euroclass E according to EN 13501-1.
Constructional data
Name Value Unit
Gross density 25 - 50 kg/m3
Compressive strength acc. to EN 826 0.2 - 0.7 N/mm2
Tensile strength acc. to EN 826 0.2 - 1 N/mm2
Modulus of elasticity acc. to EN 826 10 - 50 N/mm2
Calculation value for thermal conductivity 0.03 -
W/(mK)
EN 12667 and EN 13164 Annex C 0.035
Water vapour diffusion resistance factor acc.
50 - 250 -
to EN 12088
Creep behaviour or permanent compressive
=< 0.25 N/mm2
strength acc. to EN 1606
Water absorption after diffusion acc. to EN
1 - 3 Vol.-%
12088
Freeze-thaw resistance acc. to EN 12091 =< 1 Vol.-%
2 Environmental Product Declaration - Ravago Building Solutions - RAVATHERM™ XPS (X) extruded polystyrene foam insulation with non-halogenated blowing agents
LCA: Calculation rules
modules are declared: A1–A3, C, D and additional modules: A4
Declared Unit + A5.
The declared unit is 1 m³ of the XPS insulation product. The
declared product reflects the average of seven of Ravago's Production - Modules A1-A3
sites weighted by production volume share: The product stage includes:
• Balaton (HU); 33.07 kg/m3 (18%) • Raw material supply including secondary materials (A1)
• Rheinmuenster (DE): 34.75 kg/m3 (18%) • Transport to the manufacturer (A2): Transport is
• Lavrion (GR): 33.60 kg/m3 (17%) considered for all the input raw materials
• Schkopau (DE): 35.23 kg/m3 (17%) • Manufacturing (A3), including provision of all materials,
• Drusenheim (FR): 35.35 kg/m3 (16%) products and energy, as well as waste processing up to
the end-of-waste state.
• Artix (FR): 33.63 kg/m3 (9%)
• King's Lynn (GB): 38.08 kg/m3 (5%)
Construction stage - Modules A4-A5
The construction process stage includes:
The weighted average density of the product is 34.4 kg/m³.
• Transport to the construction site (A4)
• Treatment of packaging material (A5)
Declared unit
Name Value Unit End-of-life stage– Modules C1-C4 and D
Gross density 34.4 kg/m3 The end-of-life stage includes
Declared unit 1 m3 • Manual dismantling (Load free) (C1)
• Transport to EoL (C2)
For XPS products with densities or thicknesses different from
• Waste processing & disposal (C) with two 100 %
the reference density of 34.4 kg/m³, the environmental impacts
scenarios (scenario 1: Incineration (C3 and D); scenario
may be calculated by linear scaling using the following formula.
2: Landfill (C4))
• Reuse, recovery or recycling potential (D) - beyond
system boundary.
Geographic Representativeness
Land or region, in which the declared product system is
Iadap – adapted LCIA indicator or LCI parameter manufactured, used or handled at the end of the product´s
Iref – LCIA indicator or LCI parameter for reference density of lifespan: Europe
34.4 kg/m3
ρadap – adapted density
Comparability
ρref – reference density of 34.4 kg/m3
Basically, a comparison or an evaluation of EPD data is only
dadap – adapted board thickness
possible if all the data sets to be compared were created
dref – thickness of reference board
according to EN 15804 and the building context, respectively
the product-specific characteristics of performance, are taken
System boundary into account.
Type of EPD according to EN 15804: "cradle to gate with Background database: Sphera LCA FE (GaBi ts), CUP 2022.2
options, modules C1–C4, and module D". The following
LCA: Scenarios and additional technical information
product.
Characteristic product properties of biogenic carbon
Information on describing the biogenic Carbon Content at
factory gate
Name Value Unit Transport to the building site (A4)
kg Name Value Unit
Biogenic carbon content in product -
C Litres of fuel (per declared unit - 1m3) 0.2 l/100km
Biogenic carbon content in accompanying kg Transport distance (weighted average based on
0.00375 495 km
packaging C production volumes)
Capacity utilisation (including empty runs) 61 %
Note: 1 kg of biogenic carbon is equivalent to 44/12 kg of CO 2. Gross density of products transported 34.4 kg/m3
The transport distance can be modified to project-specific
criteria if required by linear scaling.
The following technical scenario information is required for the
declared modules and optional for non-declared modules.
The following technical information is a basis for the declared Installation into the building (A5)
modules or can be used for developing specific scenarios in the The thermal treatment of the packaging is considered in this
context of a building assessment if modules are not declared module. The following quantities are produced per 1 m3 of XPS
(MND). The values refer to the declared unit of 1 m3 XPS product (weighted average based on production volume
3 Environmental Product Declaration - Ravago Building Solutions - RAVATHERM™ XPS (X) extruded polystyrene foam insulation with non-halogenated blowing agents
shares): The transport to End of Life (C2) is calculated with a distance of
Name Value Unit 50 km (with 70 % utilization).
Packaging film (LDPE) 0.68 kg Name Value Unit
EPS Beams 0.29 kg Collected separately waste type XPS 34.4 kg
Wooden Pallet 0.01 kg Energy recovery (Scenario 1) 34.4 kg
Landfilling (Scenario 2) 34.4 kg
Reuse, recovery and/or recycling potentials (D), relevant
End of life (C1-C4)
scenario information
For the End-of-Life stage, two different scenarios are
Module D includes the credits of the thermal and electrical
considered. One scenario with 100 % incineration (scenario 1:
energy generated in Modules A5 and C3/1 due to thermal
C3/1, D1) and one scenario with 100 % landfill (scenario. 2:
treatment of packaging and product waste (XPS product).
C4/2, D2) are calculated. The incineration of XPS results in
Avoided burdens have been calculated by the inversion of
benefits beyond the system boundary (module D) due to
residual grid and thermal energy from natural gas, using
energy substitution of electricity and thermal energy under
European datasets.
European conditions.
A waste incineration plant with R1-value > 0.6 is assumed.
4 Environmental Product Declaration - Ravago Building Solutions - RAVATHERM™ XPS (X) extruded polystyrene foam insulation with non-halogenated blowing agents
LCA: Results
The following tables display the environmentally relevant results according to EN 15804 for 1 m3 XPS board. The two EoL Scenarios
are represented in modules C3/1, C4/2, D/1, and D/2. C3/1 and D/1 show the environmental results in the case of thermal treatment of
XPS products. D/1 covers also the results of the packaging treatment from Module A5. Module C4/2 reflects the landfilling of XPS (for
scenario 2, "landfilling" the values in Module D for XPS are 0). Hence, Module D/2 shows only the environmental results of the
packaging treatment from Module A5.
DESCRIPTION OF THE SYSTEM BOUNDARY (X = INCLUDED IN LCA; MND = MODULE OR INDICATOR NOT DECLARED; MNR
= MODULE NOT RELEVANT)
Benefits and
Construction loads beyond
Product stage Use stage End of life stage
process stage the system
boundaries
la ire ta m w a Ry lp p u s tro p s n a rT g n iru tc a fu n a M e h t m o rf tro p s n a rTe tis e h t o t e ta g y lb m e s s A e s U e c n a n e tn ia M ria p e R tn e m e c a lp e R tn e m h s ib ru fe R y g re n e la n o ita re p Oe s u re ta w la n o ita re p Oe s u n o itc u rts n o c -e Dn o itilo m e d tro p s n a rT g n is s e c o rp e ts a W la s o p s iD -e s u e R-y re v o c e R-g n ilc y c e Rla itn e to p
A1 A2 A3 A4 A5 B1 B2 B3 B4 B5 B6 B7 C1 C2 C3 C4 D
X X X X X MND MND MNR MNR MNR MND MND X X X X X
RESULTS OF THE LCA - ENVIRONMENTAL IMPACT according to EN 15804+A2: 1 m3 RAVATHERM™ XPS product
Parameter Unit A1-A3 A4 A5 C1 C2 C3/1 C4/2 D/1 D/2
GWP-total kg CO 2 eq 9.38E+01 3.01E+00 3.11E+00 0 2.79E-01 1.15E+02 2.44E+00 -3.68E+01 -1.56E+00
GWP-fossil kg CO 2 eq 9.38E+01 2.98E+00 3.1E+00 0 2.77E-01 1.15E+02 2.44E+00 -3.68E+01 -1.56E+00
GWP-biogenic kg CO 2 eq 3.13E-02 1.27E-02 8.17E-03 0 1.18E-03 3.44E-03 5.14E-03 -4.42E-02 -1.88E-03
GWP-luluc kg CO 2 eq 2.85E-02 1.68E-02 3.42E-06 0 1.56E-03 1.35E-04 1.19E-03 -1.61E-03 -6.81E-05
ODP kg CFC11 eq 1.94E-10 1.8E-13 1.33E-13 0 1.67E-14 4.82E-12 3.27E-12 -1.79E-10 -7.6E-12
AP mol H+ eq 1.47E-01 2.97E-03 2.99E-04 0 2.76E-04 1.01E-02 7.22E-03 -3.71E-02 -1.57E-03
EP-freshwater kg P eq 1.5E-04 8.98E-06 3.11E-08 0 8.33E-07 1.13E-06 4.55E-04 -9.21E-06 -3.91E-07
EP-marine kg N eq 3.82E-02 9.38E-04 6.37E-05 0 8.7E-05 2.22E-03 1.6E-03 -1.18E-02 -4.99E-04
EP-terrestrial mol N eq 4.18E-01 1.13E-02 1.4E-03 0 1.05E-03 4.75E-02 1.75E-02 -1.28E-01 -5.41E-03
kg NMVOC
POCP 2.28E-01 2.57E-03 1.89E-04 0 2.39E-04 6.54E-03 5.14E-03 -3.39E-02 -1.44E-03
eq
ADPE kg Sb eq 1.47E-05 2.51E-07 3.23E-09 0 2.33E-08 1.17E-07 1.69E-07 -3.03E-06 -1.29E-07
ADPF MJ 2.81E+03 4.02E+01 3.6E-01 0 3.73E+00 1.28E+01 3.46E+01 -6.83E+02 -2.9E+01
m3 world eq
WDP 1.69E+01 2.7E-02 2.78E-01 0 2.5E-03 0 -2.4E-02 -1.4E+00 -5.94E-02
deprived
GWP = Global warming potential; ODP = Depletion potential of the stratospheric ozone layer; AP = Acidification potential of land and water; EP =
Eutrophication potential; POCP = Formation potential of tropospheric ozone photochemical oxidants; ADPE = Abiotic depletion potential for non-fossil
resources; ADPF = Abiotic depletion potential for fossil resources; WDP = Water (user) deprivation potential)
RESULTS OF THE LCA - INDICATORS TO DESCRIBE RESOURCE USE according to EN 15804+A2: 1 m3 RAVATHERM™ XPS
product
Parameter Unit A1-A3 A4 A5 C1 C2 C3/1 C4/2 D/1 D/2
PERE MJ 9.9E+01 2.29E+00 2.2E-01 0 2.12E-01 3.06E+00 2.84E+00 -5.64E+01 -2.39E+00
PERM MJ 1.35E-01 0 -1.35E-01 0 0 0 0 0 0
PERT MJ 9.91E+01 2.29E+00 8.52E-02 0 2.12E-01 3.06E+00 2.84E+00 -5.64E+01 -2.39E+00
PENRE MJ 1.48E+03 4.03E+01 4.32E+01 0 3.74E+00 1.3E+03 3.46E+01 -6.83E+02 -2.9E+01
PENRM MJ 1.33E+03 0 -4.29E+01 0 0 -1.28E+03 0 0 0
PENRT MJ 2.81E+03 4.03E+01 3.6E-01 0 3.74E+00 1.28E+01 3.46E+01 -6.83E+02 -2.9E+01
SM kg 9.48E+00 0 0 0 0 0 0 0 0
RSF MJ 0 0 0 0 0 0 0 0 0
NRSF MJ 0 0 0 0 0 0 0 0 0
FW m3 4.68E-01 2.58E-03 6.5E-03 0 2.4E-04 2.2E-01 4.47E-04 -8.6E-02 -3.65E-03
PERE = Use of renewable primary energy excluding renewable primary energy resources used as raw materials; PERM = Use of renewable primary
energy resources used as raw materials; PERT = Total use of renewable primary energy resources; PENRE = Use of non-renewable primary energy
excluding non-renewable primary energy resources used as raw materials; PENRM = Use of non-renewable primary energy resources used as raw
materials; PENRT = Total use of non-renewable primary energy resources; SM = Use of secondary material; RSF = Use of renewable secondary fuels;
NRSF = Use of non-renewable secondary fuels; FW = Use of net fresh water
RESULTS OF THE LCA – WASTE CATEGORIES AND OUTPUT FLOWS according to EN 15804+A2:
1 m3 RAVATHERM™ XPS product
Parameter Unit A1-A3 A4 A5 C1 C2 C3/1 C4/2 D/1 D/2
HWD kg 1.52E-07 1.93E-10 3.38E-11 0 1.79E-11 1.2E-09 5.33E-09 -8.23E-08 -3.49E-09
NHWD kg 7.61E-01 5.77E-03 1.42E-02 0 5.36E-04 6.62E-01 3.42E+01 -1.61E-01 -6.84E-03
RWD kg 5.51E-02 4.96E-05 2.17E-05 0 4.6E-06 7.7E-04 4.25E-04 -6.38E-02 -2.71E-03
5 Environmental Product Declaration - Ravago Building Solutions - RAVATHERM™ XPS (X) extruded polystyrene foam insulation with non-halogenated blowing agents
CRU kg 0 0 0 0 0 0 0 0 0
MFR kg 0 0 0 0 0 0 0 0 0
MER kg 0 0 0 0 0 0 0 0 0
EEE MJ 3.64E-01 0 6.33E+00 0 0 2.08E+02 0 0 0
EET MJ 6.48E-01 0 1.13E+01 0 0 3.71E+02 0 0 0
HWD = Hazardous waste disposed; NHWD = Non-hazardous waste disposed; RWD = Radioactive waste disposed; CRU = Components for re-use;
MFR = Materials for recycling; MER = Materials for energy recovery; EEE = Exported electrical energy; EET = Exported thermal energy
RESULTS OF THE LCA – additional impact categories according to EN 15804+A2-optional:
1 m3 RAVATHERM™ XPS product
Parameter Unit A1-A3 A4 A5 C1 C2 C3/1 C4/2 D/1 D/2
Disease
PM 1.13E-06 1.75E-08 1.75E-09 0 1.62E-09 5.9E-08 6.94E-08 -3.24E-07 -1.38E-08
incidence
IR kBq U235 eq 8.34E+00 7.27E-03 3.56E-03 0 6.75E-04 1.26E-01 6.27E-02 -9.33E+00 -3.96E-01
ETP-fw CTUe 1.61E+03 2.79E+01 1.69E-01 0 2.59E+00 6.26E+00 3.38E+01 -1.2E+02 -5.09E+00
HTP-c CTUh 3.24E-08 5.62E-10 1.9E-11 0 5.22E-11 6.31E-10 1.52E-09 -4.47E-09 -1.89E-10
HTP-nc CTUh 1.42E-06 2.91E-08 5.99E-10 0 2.7E-09 2.05E-08 1.27E-07 -2.05E-07 -8.7E-09
SQP SQP 1.12E+02 1.38E+01 1.09E-01 0 1.28E+00 3.88E+00 2.49E+00 -3.58E+01 -1.52E+00
PM = Potential incidence of disease due to PM emissions; IR = Potential Human exposure efficiency relative to U235; ETP-fw = Potential comparative
Toxic Unit for ecosystems; HTP-c = Potential comparative Toxic Unit for humans (cancerogenic); HTP-nc = Potential comparative Toxic Unit for humans
(not cancerogenic); SQP = Potential soil quality index
Disclaimer 1 – for the indicator “Potential Human exposure efficiency relative to U235”. This impact category deals mainly with the
eventual impact of low-dose ionizing radiation on human health of the nuclear fuel cycle. It does not consider effects due to possible
nuclear accidents, occupational exposure or radioactive waste disposal in underground facilities. Potential ionizing radiation from the
soil, radon and from some construction materials is also not measured by this indicator.
Disclaimer 2 – for the indicators “abiotic depletion potential for non-fossil resources”, “abiotic depletion potential for fossil resources”,
“water (user) deprivation potential, deprivation-weighted water consumption”, “potential comparative toxic unit for ecosystems”,
“potential comparative toxic unit for humans – cancerogenic”, “Potential comparative toxic unit for humans - not cancerogenic”,
“potential soil quality index”. The results of this environmental impact indicator shall be used with care as the uncertainties on these
results are high as there is limited experience with the indicator.
References
Standards
EN 14307
CPR EN 14307:2015 Thermal insulation products for building
Regulation No. 305/2011: Construction Products Regulation of equipment and industrial installations - Factory-made extruded
the European Parliament and of the European Council, 2011. polystyrene foam (XPS) products - Specification
EN 12088 EN 1606
EN 12088:2013-06 Thermal insulating products for building EN 1606:2013-05 Thermal insulating products for building
applications. Determination of long term water absorption by applications - Determination of compressive creep
diffusion
REACH
EN 12091 Regulation (EC) No 1907/2006 of the European Parliament and
EN 12091:2013-06 of the Council of 18 December 2006 concerning the
Thermal insulating products for building applications - Registration, Evaluation, Authorisation and Restriction of
Determination of freeze-thaw resistance Chemicals (REACH)
EN 12667 BPR
EN 12667:2001 Thermal performance of building materials and Regulation (EU) No 528/2012 of the European Parliament and
products - Determination of thermal resistance by means of of the Council of 22 May 2012 concerning the making available
guarded hot plate and heat flow meter methods - Products of on the market and use of biocidal products
high and medium thermal resistance
EN 15804
EN 13164 + A1 EN 15804:2012+A2:2019+AC:2021, Sustainability of
EN 13164:2012 + A1:2015 Thermal insulation products for construction works — Environmental Product Declarations -
buildings - Factory-made extruded polystyrene foam (XPS) Core rules for the product category of construction products.
products - Specification
Further References
EN 13501
EN 13501-1:2019-05 Fire classification of construction products GaBi ts
and building elements - Part 1: Classification using data from GaBi ts dataset documentation for the software-system and
reaction to fire tests databases, LBP, University of Stuttgart and thinkstep,
Leinfelden-Echterdingen, 2023 (https://www.gabi-
ISO 14025 software.com/support/gabi)
EN ISO 14025:2011, Environmental labels and declarations
Type III environmental declarations — Principles and IBU 2021
procedures. Institut Bauen und Umwelt e.V.: General Instructions for the
6 Environmental Product Declaration - Ravago Building Solutions - RAVATHERM™ XPS (X) extruded polystyrene foam insulation with non-halogenated blowing agents
EPD programme of Institut Bauen und Umwelt e.V., Version Institut Bauen und Umwelt e.V., 2021.
2.0, Berlin: Institut Bauen und Umwelt e.V., 2021
(www.ibu-epd.com) PCR Part B
PCR - Part B: Requirements of the EPD for Insulating materials
PCR Part A made of foam plastics, v8, Institut Bauen und Umwelt e.V.,
PCR - Part A: Calculation rules for the Life Cycle Assessment 2023.
and Requirements on the Background Report, version 1.3, .
7 Environmental Product Declaration - Ravago Building Solutions - RAVATHERM™ XPS (X) extruded polystyrene foam insulation with non-halogenated blowing agents
Publisher
Institut Bauen und Umwelt e.V. +49 (0)30 3087748- 0
Hegelplatz 1 info@ibu-epd.com
10117 Berlin www.ibu-epd.com
Germany
Programme holder
Institut Bauen und Umwelt e.V. +49 (0)30 3087748- 0
Hegelplatz 1 info@ibu-epd.com
10117 Berlin www.ibu-epd.com
Germany
Author of the Life Cycle Assessment
Sphera Solutions GmbH +49 711 341817-0
Hauptstraße 111- 113 info@sphera.com
70771 Leinfelden-Echterdingen www.sphera.com
Germany
Owner of the Declaration
RBS Germany GmbH -
Value Park Y51 info.de.rbs@ravago.com
06258 Schkopau www.ravagobuildingsolutions.com
Germany
8 Environmental Product Declaration - Ravago Building Solutions - RAVATHERM™ XPS (X) extruded polystyrene foam insulation with non-halogenated blowing agents
