ver1 2015
ENVIRONMENTAL PRODUCT DECLARATION
in accordance with ISO 14025, ISO 21930 and EN 15804
Owner of the declaration: BM Vallá
Program operator: The Norwegian EPD Foundation
Publisher: The Norwegian EPD Foundation
Declaration number: NEPD-2365-1103-EN
Registration number: NEPD-2365-1103-EN
ECO Platform reference number: -
Issue date: 08.09.2020
Valid to: 08.09.2025
Ready mix concrete C30/C37 outdoor
BM Vallá
www.epd-norge.no
NEPD-2365-1103-EN Ready mix concrete C30/C37 outdoor (korr090221)
1 / 8
General information
Product: Owner of the declaration:
Ready mix concrete C30/C37 outdoor
BM Vallá
Contact person: Smári Valgarðsson
Phone: +3546175020
e-mail: smariva@bmvalla.is
Program operator: Manufacturer:
BM Vallá
The Norwegian EPD Foundation
Bildshøfdi 7 , 110 Reykjavik, Iceland
Pb. 5250 Majorstuen, 0303 Oslo
Iceland
Phone: +47 23 08 80 00
e-mail: post@epd-norge.no
Declaration number: Place of production:
BM Vallá
NEPD-2365-1103-EN Bildshøfdi 7 , 110 Reykjavik, Iceland
Iceland
ECO Platform reference number: Management system:
ISO 9001
This declaration is based on Product Category Rules: Organisation no:
10480
CEN Standard EN 15804:2012+A1:2013 serves as core PCR
NPCR 020:2018 Part B for Concrete and concrete elements
Statement of liability: Issue date:
The owner of the declaration shall be liable for the underlying information and 08.09.2020
evidence. EPD Norway shall not be liable with respect to manufacturer
information, life cycle assessment data and evidences. Valid to:
08.09.2025
Declared unit: Year of study:
1 m3 Ready mix concrete C30/C37 outdoor 2020
Declared unit with option: Comparability:
EPD of construction products may not be comparable if they not comply with EN
A1,A2,A3,A4
15804 and seen in a building context.
Functional unit: Development and verification of EPD:
The declaration has been developed and verified using EPD tool lca.tools
ver EPD2020.11, developed by LCA.no AS. The EPD tool is integrated into
the company's environmental management system, and has been
approved by EPD-Norway
General information on verification of EPD from EPD tools:
Independent verification of data, other environmental information and Developer of EPD:
the declaration according to ISO 14025:2010, § 8.1.3 and § 8.1.4. Individual
third party verification of each EPD is not required when the EPD tool is i) Smari Valgardsson
integrated into the company's environmental management system, ii) the
procedures for use of the EPD tool are approved by EPDNorway, and iii) Reviewer of company-specific input data and EPD:
the proccess is reviewed annualy. See Appendix G of EPD-Norway's
General Programme Instructions for further information on EPD tools. Einar Einarsson
Verification of EPD tool: Approved:
Independent third party verification of the EPD tool, background data
Sign
and test-EPD in accordance with EPDNorway's procedures and guidelines
for verification and approval of EPD tools.
Anne Rønning, Norsus AS
(no signature required) Håkon Hauan, CEO EPD-Norge
NEPD-2365-1103-EN Ready mix concrete C30/C37 outdoor (korr090221)
2 / 8
Product
Product description: Technical data:
Ready mix concrete for outdoor use, produced according to ÍST-EN C30/37-25; XC4 XF2/XF3 XS1
206:2013+A1:2016
Dmax 25 - Air >5% - v/s < 0,50
Product specification
Market:
Iceland
Materials kg % Reference service life, product
Cement 350,00 15,23
Same as for buildings
Aggregate 1780,00 77,43
Reference service life, building
Water 165,00 7,18
Chemicals 3,75 0,16 60 years
Total 2298,75
LCA: Calculation rules
Declared unit: Allocation:
The allocation is made in accordance with the provisions of EN 15804.
1 m3 Ready mix concrete C30/C37 outdoor
Incoming energy and water and waste production in-house is allocated
Cut-off criteria: equally among all products through mass allocation. Effects of primary
production of recycled materials is allocated to the main product in
All major raw materials and all the essential energy is included. The
which the material was used. The recycling process and transportation of
production processes for raw materials and energy flows with very small
the material is allocated to this analysis.
amounts (less than 1%) are not included. These cut-off criteria do not
apply for hazardous materials and substances.
Data quality:
Specific data for the product composition are provided by the manufacturer. They represent the production of the declared product and were collected for
EPD development in the year of study. Background data is based on registered EPDs according to EN 15804, Ostfold Research databases, ecoinvent and other
LCA databases. The data quality of the raw materials in A1 is presented in the table below.
Materials Source Data quality Year
Chemicals EPD-EFC-20150086-IAG1-EN EPD 2015
Chemicals EPD-EFC-20150091-IAG1-EN EPD 2015
Water ecoinvent 3.4 Database 2017
Aggregate Supplier specific data Database 2019
Cement NEPD-2277-1028-NO EPD 2020
NEPD-2365-1103-EN Ready mix concrete C30/C37 outdoor (korr090221)
3 / 8
System boundary:
Additional technical information:
NEPD-2365-1103-EN Ready mix concrete C30/C37 outdoor (korr090221)
4 / 8
LCA: Scenarios and additional technical information
The following information describe the scenarios in the different modules of the EPD.
Transport from production place to user (A4)
Capacity utilisation Fuel/Energy
Type Type of vehicle Distance km Unit Value (l/t)
(incl. return) % consumption
Truck 53,0 % Concrete truck, EURO 6 14 0,020216 l/tkm 0,28
Railway l/tkm
Boat l/tkm
Other Transportation l/tkm
NEPD-2365-1103-EN Ready mix concrete C30/C37 outdoor (korr090221)
5 / 8
LCA: Results
The LCA results are presented below for the declared unit defined on page 2 of the EPD document.
System boundaries (X=included, MND=module not declared, MNR=module not relevant)
Construction Beyond the
Product stage installation User stage End of life stage . system
stage bondaries
A1 A2 A3 A4 A5 B1 B2 B3 B4 B5 B6 B7 C1 C2 C3 C4 . D
X X X X MND MND MND MND MND MND MND MND MND MND MND MND . MND
Environmental impact
Parameter Unit A1 A2 A3 A4
GWP kg CO 2 -eq 2,62E+02 3,44E+01 2,03E+00 1,18E+00
ODP kg CFC11 -eq 2,08E-06 4,31E-06 3,22E-07 2,24E-07
POCP kg C 2H 4-eq 2,90E-02 3,71E-03 3,87E-04 2,10E-04
AP kg SO 2 -eq 3,65E-02 1,00E-01 1,37E-02 4,17E-03
EP kg PO 3- -eq 1,15E-01 1,49E-02 2,92E-03 8,68E-04
4
ADPM kg Sb -eq 3,53E-05 4,29E-05 1,14E-06 2,62E-06
ADPE MJ 6,16E+02 3,30E+02 2,61E+01 1,81E+01
GWP Global warming potential; ODP Depletion potential of the stratospheric ozone layer; POCP Formation potential of tropospheric photochemical oxidants;
AP Acidification potential of land and water; EP Eutrophication potential; ADPM Abiotic depletion potential for non fossil resources; ADPE Abiotic depletion
potential for fossil resources
Reading example: 9,0 E-03 = 9,0*10-3 = 0,009
*INA Indicator Not Assessed
waR slairetam tropsnarT gnirutcafunaM tropsnarT ylbmessA esU ecnanetniaM riapeR tnemecalpeR tnemhsibrufeR lanoitarepO ygrene esu lanoitarepO esu
retaw
-eD noitcurtsnoc noitilomed tropsnarT etsaW gnissecorp lasopsiD -yrevoceR-esueR -gnilcyceR laitnetop
NEPD-2365-1103-EN Ready mix concrete C30/C37 outdoor (korr090221)
6 / 8
Resource use
Parameter Unit A1 A2 A3 A4
RPEE MJ 2,28E+02 6,58E+00 2,38E+01 2,78E-01
RPEM MJ 0,00E+00 0,00E+00 0,00E+00 8,51E-02
TPE MJ 2,28E+02 6,58E+00 2,38E+01 3,63E-01
NRPE MJ 6,35E+02 3,42E+02 2,65E+01 1,85E+01
NRPM MJ 6,99E+00 0,00E+00 0,00E+00 0,00E+00
TRPE MJ 6,42E+02 3,42E+02 2,65E+01 1,85E+01
SM kg 5,01E+01 0,00E+00 0,00E+00 0,00E+00
RSF MJ 3,61E+02 0,00E+00 0,00E+00 0,00E+00
NRSF MJ 4,59E+02 0,00E+00 0,00E+00 0,00E+00
W m3 3,19E-01 7,65E-02 1,20E-01 1,65E-02
RPEE Renewable primary energy resources used as energy carrier; RPEM Renewable primary energy resources used as raw materials; TPE Total use of renewable
primary energy resources; NRPE Non renewable primary energy resources used as energy carrier; NRPM Non renewable primary energy resources used as
materials; TRPE Total use of non renewable primary energy resources; SM Use of secondary materials; RSF Use of renewable secondary fuels; NRSF Use of non
renewable secondary fuels; W Use of net fresh water
Reading example: 9,0 E-03 = 9,0*10-3 = 0,009
*INA Indicator Not Assessed
End of life - Waste
Parameter Unit A1 A2 A3 A4
HW kg 2,86E-04 1,90E-04 1,50E-05 1,40E-05
NHW kg 2,20E+01 2,73E+01 2,78E-01 1,83E+00
RW kg INA* INA* INA* INA*
HW Hazardous waste disposed; NHW Non hazardous waste disposed; RW Radioactive waste disposed
Reading example: 9,0 E-03 = 9,0*10-3 = 0,009
*INA Indicator Not Assessed
End of life - Output flow
Parameter Unit A1 A2 A3 A4
CR kg 0,00E+00 0,00E+00 0,00E+00 0,00E+00
MR kg 0,00E+00 0,00E+00 0,00E+00 0,00E+00
MER kg 0,00E+00 0,00E+00 0,00E+00 0,00E+00
EEE MJ INA* INA* INA* INA*
ETE MJ INA* INA* INA* INA*
CR Components for reuse; MR Materials for recycling; MER Materials for energy recovery; EEE Exported electric energy; ETE Exported thermal energy
Reading example: 9,0 E-03 = 9,0*10-3 = 0,009
*INA Indicator Not Assessed
NEPD-2365-1103-EN Ready mix concrete C30/C37 outdoor (korr090221)
7 / 8
Additional Norwegian requirements
Greenhouse gas emissions from the use of electricity in the manufacturing phase
National production mix from import, low voltage (production of transmission lines, in addition to direct emissions and losses in grid) of applied electricity for
the manufacturing process (A3).
Electricity mix Data source Amount Unit
El-mix Iceland (kWh) Ecoinvent 3.6 50,38 g CO2-ekv/kWh
Dangerous substances
The product contains no substances given by the REACH Candidate list or the Norwegian priority list.
Indoor environment
Bibliography
ISO 14025:2010 Environmental labels and declarations - Type III environmental declarations - Principles and procedures.
ISO 14044:2006 Environmental management - Life cycle assessment - Requirements and guidelines.
EN 15804:2012+A1:2013 Environmental product declaration - Core rules for the product category of construction products.
ISO 21930:2017 Sustainability in buildings and civil engineering works - Core rules for environmental product declarations of construction products.
ecoinvent v3, Allocation, cut-off by classification, Swiss Centre of Life Cycle Inventories.
Iversen et al., (2018) eEPD v3.0 - Background information for EPD generator system. LCA.no report number 04.18
Vold, M. og Edvardsen, T. (2014) EPD-generator for betongindustrien, bakgrunnsinformasjon for verifisering, OR 04.14.
NPCR Part A: Construction products and services. Ver. 1.0. April 2017, EPD-Norge.
NPCR 020 Part B for Concrete and concrete elements. Ver. 2.0 October 2018, EPD-Norge.
Program operator and publisher Phone: +47 23 08 80 00
The Norwegian EPD Foundation e-mail: post@epd-norge.no
Post Box 5250 Majorstuen, 0303 Oslo,Norway web: www.epd-norge.no
Owner of the declaration Phone: +3546175020
BM Vallá e-mail: smariva@bmvalla.is
Bildshøfdi 7 , 110 Reykjavik, Iceland web: www.bmvalla.is
Author of the Life Cycle Assessment Phone: +47 69 35 11 00
Østfoldforskning AS e-mail: post@ostfoldforskning.no
Stadion 4 , 1671 Kråkerøy web: www.ostfoldforskning.no
Developer of EPD generator Phone: +47 916 50 916
LCA.no AS e-mail: post@lca.no
Dokka 1C,1671 Kråkerøy web: www.lca.no
NEPD-2365-1103-EN Ready mix concrete C30/C37 outdoor (korr090221)
8 / 8
