Environmental Product
Declaration
In accordance with ISO 14025 and EN 15804 +A2
ROCKWOOL Norden
Owner of the declaration: Product name:
ROCKWOOL Nordics
ROCKWOOL® stone wool
Program holder and publisher: thermal insulation
The Norwegian EPD foundation
TOPROCK System for
Declaration number: the Scandinavian market
Manufacturer
The Norwegian NReEgPiDst-3ra4t1i1o-n2 N02u4m-EbNer: ROCKWOOL Nordics
EPD Foundation
NIsEsPuDe -d3a4t1e1: -2024-EN
Valid to:
24.03.2022
24.03.2027
General information
Product: Owner of the declaration:
ROCKWOOL® stone wool thermal insulation, ROCKWOOL Nordics
TOPROCK System for the Scandinavian market Contact person: Christian J. Kofod
Phone: +45 4656 1616
Program Operator: e-mail: christian.kofod@rockwool.com
The Norwegian EPD Foundation
Manufacturer:
Post Box 5250 Majorstuen, 0303 Oslo, Norway
Tlf: +47 23 08 80 00 ROCKWOOL Nordics,
e-mail: post@epd-norge.no Hovedgaden 501, DK-2640 Hedehusene
Phone: +45 4656 1616
Declaration Number: e-mail: info@rockwool.com
Place of production:
NEPD-3411-2024-EN Doense factory (Biomethane line), Denmark
This declaration is based on Product
Doense factory (Conventional line), Denmark
Category Rules:
Vamdrup factory (Biomethane), Denmark
CEN Standard EN 15804+A2 serves as core PCR
NPCR Part A Construction products and services Management system:
NPCR 012:2018 version 2. Part B for Thermal
ISO 14001, ISO 9001
insulation products
Organisation no:
Statements:
CVR. nr. 42391719
The owner of the declaration shall be liable for the
underlying information and evidence. EPD
Issue date:
Norway shall not be liable with respect to
manufacturer, life cycle assessment data and
evidences.
2V4a.l0i3d. 2t0o2: 2
Declared unit:
1 m2 of stone wool thermal insulation with a
2Y4e.a0r3 .o20f 2s7tudy:
thermal resistance (R) of 1,0 m2K/W.
2021
Functional unit:
1 m2 of stone wool thermal insulation with a Comparability:
thermal resistance (R) of 1,0 m2K/W with a EPDs of construction products may not be
reference service life of minimum 60 years. comparable if they are not compliant with EN
15804:A2:2019 and not seen in a building context.
Verification:
Independent verification of the declaration and The EPD has been worked out by:
data, according to ISO14025:2010
Larisa Xanthopoulou, ROCKWOOL Int. A/S
internal external
Jane Anderson
Independent verifier approved by EPD Norway Approved (Manager of EPD Norway)
EPD for the best environmental decision 2
Product
Description of the product and use of the EPD:
This EPD documents the potential environmental impacts of 1m2 of ROCKWOOL® TOPROCK
System stone wool insulation with a thermal resistance (R-value) equal to 1 m2K/W. The
intended use of the EPD is to communicate quantified environmental impacts of construction
products for application in the assessment of the environmental performance of buildings.
ROCKWOOL® stone wool thermal insulation is a durable and firesafe insulation material that
can be used to insulate against against heat, cold, fire, vibrations and noise.
ROCKWOOL® stone wool is made primarily from abundantly available volcanic rock, an
increasing proportion of recycled ROCKWOOL® stone wool material and a cured resin binder.
Other materials utilised in the production of ROCKWOOL® stone wool are by-products from
other industries. Since 2012, ROCKWOOL® has been offering a take back system for closed loop
recycling – Rockcycle.
The product covered by this declaration is ROCWKOOL® TOPROCK System produced for the
Scandinavian market (Denmark, Norway and Sweden). The unfaced and uncoated synthetic
resin-bonded stone wool materials described in this declaration are produced in the form of a
batt. The density of the product as installed will vary according to end use insulation
requirements. Average density as installed: 75 kg/m3
ROCKWOOL® stone wool is a non-combustible material that does not react to fire. Stone wool’s
built-in fire protection is natural and not dependent on flame retardants. Stone wool withstands
temperatures exceeding 1,000 degrees Celsius, and retains its fire performance throughout its
lifetime.
The insulation properties of stone wool is primarily achieved by the immobile air within in the
open structure of the product. Therefore, the declared insulation property will remain constant
for the declared lifetime of the product. This also allows the product to absorb noise and sounds
and contribute to a better indoor acoustic climate.
ROCKWOOL® stone wool fibers are proven to be safe to manufacture, install and live with.
Health and safety installation instructions shall always be followed. ROCKWOOL® stone wool
fibers comply with the European REACH regulation and do not have any health-related
classifications or negative impact on the indoor environment.
The packaging is included in the assessment.
Product specification:
The average composition used for this EPD is calculated based on average factory consumption
figures for raw materials.. The raw materials are mainly non-scarce stones, and resin binder.
Materials %
Mineral Wool >95%
De-duster and water repellency oil <1%
Binder <5%
EPD for the best environmental decision 3
Technical data:
For the products covered by this EPD, the performance data are in accordance with the
declaration of performance with respect to its essential characteristics according to EN
13162:2012+A1:2015, "Thermal insulation products for buildings – Factory made mineral wool
(MW) products – Specification".
A full overview of the technical specifications can be found on www.rockwool.com/dk
Declared Performance Norms
Thermal
0,039 W/mK EN 12939 and EN 12667
conductivity
Fire class A2-S1,d0 EN 13501-1:2007+ A1:2009
Market:
This EPD is intended for the Nordic markets (A4 module can be adjusted with scaling factors
provided to reflect correct transportation distance).
Reference service life, product:
ROCKWOOL® stone wool thermal insulation products are extremely durable and provide
effective performance for the lifetime of a building or host structure, with no need to be
replaced. The thermal, fire-resistance, and acoustic performance of ROCKWOOL® stone wool
products, when correctly installed, remains the same during 60 years reference service life or as
long as the insulation is part of the building.
Reference service life, building:
In this EPD, the reference service life of a building is set to 60 years.
EPD for the best environmental decision 4
LCA: Calculation rules
1m2 of ROCKWOOL® TOPROCK System with a thermal resistance
Declared unit
RD=1 m2K/W.
Density of reference product 75 kg/m3
Thickness of reference product 39 mm
Scope Cradle to Grave
Reference service life 60 years
Energy used for manufacturing process Renewable electricity mix GO’s from Danish wind power, to be
- Electricity prolonged to be valid at least equal to the validity of this EPD.
- Gas Biogas (Danish biomethane)
- Fossil Coke
Declared unit:
The specific product, referred to in the declared unit is 1m2 of an ROCKWOOL® TOPROCK
System stone wool batt with a thermal resistance R=1m2K/W. The reference product is 39 mm
thick with a density of 75 kg/m3. The weight of the reference product corresponding to the
declared unit is 2,9 kg.
The impact indicators for specific thicknesses can be calculated by multiplying the results of the
EPD with the respective scaling factor from a range of products covered by this EPD. A table
with the different products available in the portfolio and their respective scaling factors is
provided within the ‘Additional technical information’ section.
Data quality:
All data represents the applicable geography, time and technology for the specific and generic
data, generally assessed as good and very good. Primary data are collected from respective
production sites in Doense and Vamdrup, Denmark, in the reference year 2021 and represent
stabilized production. Generic data is from GaBi database (version 2021) with GaBi Software
version 10.0.1.92.
Allocation:
The allocation is made in accordance with the provisions of EN 15804+A2. Production activities,
electricity and energy consumption and waste generation are allocated equally among all
products from the production site through mass allocation.
EPD for the best environmental decision 5
System boundary:
The LCA is performed as a ‘cradle-to-grave ’ study, addressing all life cycle stages identified in
the EN 15804+A2. All major raw materials, energy, electricity use and waste are included for all
life cycle modules, see flowchart below. Use stage B1-7 modules are considered but are not
relevant, as there are no activities and no significant environmental impact in the use stage.
Cut-off criteria:
All major raw materials and all the essential energy are included. All hazardous materials and
substances are considered in the inventory. Data sets within the system boundary are complete
and fulfil criteria for the exclusion of inputs and output criteria. All data, materials and energy
consumptions , have been specified according to the production data and have been considered
within the inventory analysis
EPD for the best environmental decision 6
LCA: Scenarios and additional technical information
The following information describe the scenarios in the different modules of the EPD. The EPD
is based on LCA inventory data from the 2 factories. The reference flow is a weighted average
based on the distribution of production capacity of the specific product between the 2 factories.
For Doense factory, distribution of production capacity between biomethane and conventional
line for the specific product is also accounted for in the weighted average.
Transport from production place to assembly/user (A4)
Capacity utilisation (incl. Type of Fuel/Energy value
Type Distance KM
return) % vehicle consumption (l/t)
Euro 6, with
Diesel:
Truck 30 % a 27t 285 5,41 l/t
0,019 l/tkm
payload
The A4 distance is calculated as a weighted average distance for the Nordic market.
Additional distances estimated for specific markets are given in the table below
Market Distance A4, GWP fossil
Denmark 212 km 5,53E-02 kg CO2 eq
Norway 300 km 7,82E-02 kg CO2 eq
Sweden 398 km 1,04E-01 kg CO2 eq
Assembly (A5)
Unit Value
Auxiliary Kg 0
Water consumption m3 0
Electricity consumption kWh 0
Other energy carriers MJ 0
Material loss Kg 2%
Cardboard and paper packaging Kg 0,00013
Plastic packaging Kg 0,026
Wood packaging Kg 0,07
In A5 the default installation is assumed to be manual, therefore no energy consumption or
ancillary equipment is needed. The product waste from installation is assumed to be 2% and
according to the modularity principle of EN 15804+A2 its impacts are fully allocated to A5,
following same EoL scenario as in C. The A5 module includes also the corresponding end-of-life
considerations for packaging (10 % landfill). The credits from heat and electricity recovery from
incineration or material recycling from module A5 (90% recycling and energy recovery) are
attributed to module D.
EPD for the best environmental decision 7
Use stage (B1, B2, B3, B4, B5, B6, B7)
There are no consumables and no maintenance (B2), repair (B3), replacements (B4) or
refurbishments (B5) required during the use of ROCKWOOL® thermal insulation products in
standard conditions. They do not use energy (B6) or water (B7) during their operational life. No
significant emissions to the indoor environment occur in module (B1). Therefore, modules B1-
B7 are not relevant for this EPD.
End of Life (C1, C3, C4)
Unit Value
Hazardous waste disposed % 0
Collected as mixed construction waste % 100
Reuse % 0
Recycling % 7
Energy recovery % 0
To landfill % 0,93
ROCKWOOL stone wool insulation can be recycled via RockCycle or local recycling offerings.
Transport to waste processing (C2)
Capacity utilisation (incl. Type of Fuel/Energy value
Type Distance KM
Return) % vehicle consumption (l/t)
Truck, with
Truck, Diesel:
50% 17,3 t 100 km 2,5 l/t
Euro 6 0,025 l/tkm
payload
The distance represents an average distance to waste treatment facility or landfill.
Benefits and loads beyond the system boundaries (D)
Unit Value
Packaging recycled kg 0,03
Energy recovered MJ 0,7
Stone wool for recycling kg 0,2
Benefits in module D are created from packaging materials treatment (recycled meterials and
recoverd energy) after installation and recycling potential of stone wool in the end of life.
Recycling potential of net stone wool material is considered here.
EPD for the best environmental decision 8
Additional technical information
Below a list of ROCKWOOL TOPROCK System thickness’ covered by this EPD and their scaling
factors. The scaling factor can be used to estimate the environmental performance indicators for
the specific products.
System boundaries (X=included, MND= module not declared, MNR=module not relevant)
Benefits &
Product stage Construction loads beoyond
Use stage End of life stage
stage system
boundary
EPD for the best environmental decision 9
slairetam
waR
tropsnarT
gnirutcafunaM
tropsnarT ylbmessA
esU
ecnanetniaM
riapeR
tnemecalpeR tnemhsibrufeR
esu
ygrene
lanoitarepO
esu
retaw
lanoitarepO
noitilomed
noitcurtsnoc-eD
tropsnarT
gnissecorp
etsaW
lasopsiD
-gnilcyceR-yrevoceR-esueR
laitnetop
Thickness R [m2K/W] Scaling factor per m2 Scaling factor per m3
39 1 1 26
230 5,9 5,9 26
250 6,4 6,3 25
280 7,2 6,9 25
310 7,95 7,5 24
360 9,25 8,6 24
430 11,05 10,0 23
530 13,6 12,2 23
LCA: Results
A1 A2 A3 A4 A5 B1 B2 B3 B4 B5 B6 B7 C1 C2 C3 C4 D
X X X X X MNR MNR MNR MNR MNR MNR MNR X X X X X
How to read scientific notation
Scientific notation Decimal form
1,00E-01 0,1
1,00E-02 0,01
1,00E-03 0,001
1,00E-04 0,0001
1,00E-05 0,00001
Core environmental impact indicators
Indicator Unit A1-3 A4 A5 B1-B7 C1 C2 C3 C4 D
kg CO2 2,03E+00 1,04E-01 2,28E-01 MNR 0 1,02E-02 0 4,07E-02 -7,92E-02
eq.
GWP-total Global Warming Potential-total is the sum of GWP-fossil, GWP-biogenic and GWP luluc.
GWP measures the Carbon Dioxide (CO2) and other greenhouse gas emissions associated with the
product
kg CO2 2,19E+00 1,03E-01 6,26E-02 MNR 0 1,01E-02 0 4,06E-02 -8,79E-02
GWP-fossil eq. GWP-fossil takes into account the GWP of greenhouse gas emissions from fossil fuels or fossil carbon
containing substances (e.g. combustion, landfilling, etc.).
kg CO2 -1,64E-01 0,00E+00 1,65E-01 MNR 0 0,00E+0 0 0,00E+00 8,78E-03
GWP- eq.
biogenic GWP-biogenic represents the atmospheric CO2 absorbed from biomass growth and emitted during e.g.
incineration or natural decay.
kg CO2 1,09E-03 8,47E-04 4,26E-05 MNR 0 8,31E-05 0 1,19E-04 -2,99E-05
GWP- eq.
LULUC GWP-land use and land use change (luluc) takes into account greenhouse gas emissions from changes
in carbon stock as a result of land use and land use change, e.g. deforestation
kg 6,81E-09 1,32E-17 3,22E-10 MNR 0 1,29E-18 0 1,58E-16 -6,92E-15
ODP CFC11 The Ozone Depletion Potential, describes the potential for degradation of the ozone layer. High ODP
eq.
substances are forbidden today.
mol H⁺ 2,50E-02 9,18E-05 5,53E-04 MNR 0 1,06E-05 0 2,90E-04 -2,27E-04
AP eq.
The Acidification Potential reflects the potential to cause the acid deposition or “acid rain”
kg P eq. 1,48E-05 1,89E-06 4,60E-07 MNR 0 3,01E-08 0 6,81E-08 -9,79E-08
EP-
freshwater Eutrophication Potential-freshwater represents potential excessive growth of algae and damage of the
ecosystems from nutrients emissions reaching the fresh water end compartment.
kg N 3,00E-03 2,70E-05 8,00E-05 MNR 0 3,51E-06 0 7,52E-05 -4,95E-05
EP-marine eq.
As above, but emitted to the marine end compartment.
mol N 9,44E-02 3,28E-04 2,08E-03 MNR 0 4,16E-05 0 8,24E-04 -5,39E-04
EP- eq.
terrestrial Eutrophication Potential-terrestrial. Indicator for enrichment of terrestrial ecosystems w. nitrogen
based nutrients, e.g. ammonia.
kg 6,47E-03 7,80E-05 1,77E-04 MNR 0 9,31E-06 0 2,27E-04 -1,55E-04
POCP NMVOC
eq. Photochemical Ozone Creation Potential, most commonly manifested as smog.
kg Sb 6,03E-07 7,86E-09 1,38E-08 MNR 0 7,72E-10 0 3,83E-09 -1,46E-08
ADP-M&M eq. Abiotic Depletion Potential for non-fossil resources (minerals and metals); relates to the consumption
and scarcity of minerals and metals.
MJ 2,18E+01 1,38E+00 6,47E-01 MNR 0 1,35E-01 0 5,40E-01 -2,07E+00
ADP-fossil Abiotic Depletion Potential for fossil resources (oil, gas, coal). Indicator for the depletion of fossil
resources for energy use or as feedstock for the petrochemical industry.
m³ 2,45E-01 8,96E-04 2,24E-02 MNR 0 8,81E-05 0 4,36E-03 -2,76E-02
WDP Water Deprivation Potential, a “water scarcity footprint” indicator for the potential impact of water
use , linked to water deficiency to downstream human users and ecosystems
GWP-total: Global Warming Potential; GWP-fossil: Global Warming Potential fossil fuels; GWP-biogenic: Global
Warming Potential biogenic; GWP-LULUC: Global Warming Potential land use and land use change; ODP: Depletion
potential of the stratospheric ozone layer; AP: Acidification potential, Accumulated Exceedance; EP-freshwater:
Eutrophication potential, fraction of nutrients reaching freshwater end compartment; See “additional Norwegian
requirements” for indicator given as PO4 eq. EP-marine: Eutrophication potential, fraction of nutrients reaching
freshwater end compartment; EP-terrestial: Eutrophication potential, Accumulated Exceedance; POCP: Formation
potential of tropospheric ozone; ADP-M&M: Abiotic depletion potential for non-fossil resources (minerals and metals);
ADP-fossil: Abiotic depletion potential for fossil resources; WDP: Water deprivation potential, deprivation weighted
water counsumption
Reading example: 9,0 E-03 = 9,0*10-3 = 0,009
EPD for the best environmental decision 10
Additional environmental impact indicators
Indicator Unit A1-3 A4 A5 B1-B7 C1 C2 C3 C4 D
Disease
1,99E-07 5,82E-10 4,39E-09 MNR 0 6,13E-11 0 3,59E-09 -3,41E-09
incidence
PM
Particulate Matter. An indicator for potential disease incidences (occurrences) linked to emissions of
particulate matter from, e.g. diesel engines.
kBq U235 2,04E-02 2,39E-04 2,50E-03 MNR 0 2,34E-05 0 5,94E-04 -1,67E-03
IRP eq. Ionising radiation Potential, relates to the possible damage to human health from exposure to low level
radiation linked to generation of nuclear energy only.
CTUe 6,48E+00 9,94E-01 2,26E-01 MNR 0 9,76E-02 0 3,07E-01 -8,87E-02
ETP-fw Ecotoxicity Potential-freshwater. Potential toxic effects on freshwater species of emissions of
substances/chemicals.
CTUh 2,47E-09 2,01E-11 5,47E-11 MNR 0 1,97E-12 0 4,53E-11 -1,10E-11
HTP-c Human toxicity potential - cancer effects. Potential carcinogenic impacts on people from the emissions of
substances and chemicals
CTUh 1,63E-08 1,03E-09 7,67E-10 MNR 0 1,02E-10 0 4,99E-09 -4,41E-10
HTP-nc Human toxicity Potential - non-cancer effects. Potential toxic effects on humans other than carcinogenic
from the emission of substances and chemicals.
Dimension- 3,43E+01 4,73E-01 7,23E-01 MNR 0 4,63E-02 0 1,09E-01 -1,80E+00
SQP less Soil Quality Potential. Indicator representing factors impacting soil quality, e.g. Erosion, filtration ability
and groundwater regeneration.
PM: Particulate matter emissions; IRP: Ionising radiation, human health; ETP-fw: Ecotoxicity (freshwater);
ETP-c: Human toxicity, cancer effects; HTP-nc: Human toxicity, non-cancer effects; SQP: Land use related
impacts / soil quality
EPD for the best environmental decision 11
Classification of disclaimers to the declaration of core and additional environmental impact indicators
ILCD classification Indicator Disclaimer
Global warming potential (GWP) None
ILCD type / level 1 Depletion potential of the stratospheric ozone layer (ODP) None
Potential incidence of disease due to PM emissions (PM) None
Acidification potential, Accumulated Exceedance (AP) None
Eutrophication potential, Fraction of nutrients reaching freshwater end compartment (EP-freshwater) None
Eutrophication potential, Fraction of nutrients reaching marine end compartment (EP-marine) None
ILCD type / level 2
Eutrophication potential, Accumulated Exceedance (EP-terrestrial) None
Formation potential of tropospheric ozone (POCP) None
Potential Human exposure efficiency relative to U235 (IRP) 1
Abiotic depletion potential for non-fossil resources (ADP-minerals&metals) 2
Abiotic depletion potential for fossil resources (ADP-fossil) 2
Water (user) deprivation potential, deprivation-weighted water consumption (WDP) 2
ILCD type / level 3 Potential Comparative Toxic Unit for ecosystems (ETP-fw) 2
Potential Comparative Toxic Unit for humans (HTP-c) 2
Potential Comparative Toxic Unit for humans (HTP-nc) 2
Potential Soil quality index (SQP) 2
Disclaimer 1 – This impact category deals mainly with the eventual impact of low dose ionizing radiation on human health of the nuclear fuel cycle. It does not consider effects due
to possible nuclear accidents, occupational exposure nor due to radioactive waste disposal in underground facilities. Potential ionizing radiation from the soil, from radon and from
some construction materials is also not measured by this indicator.
Disclaimer 2 – The results of this environmental impact indicator shall be used with care as the uncertainties on these results are high or as there is limited experienced with the
indicator
EPD for the best environmental decision 12
Resource use
Indicator Unit A1-3 A4 A5 B1-B7 C1 C2 C3 C4 D
MJ 3,69E+01 7,69E-02 8,36E-01 MNR 0 7,53E-03 0 7,26E-02 -4,19E-01
RPEE Renewable Primary Energy used as Energy carrier only.
Typically renewable energy from Biomethane, windmills or hydropower
MJ 1,91E+00 0,00E+00 -5,74E-02 MNR 0 0,00E+00 0 0,00E+00 0,00E+00
RPEM Renewable primary energy resources used as raw materials – indicates the consumption of energy resources as
raw materials e.g. wood, or biomethane as feedstock for bio-plastics
MJ 3,88E+01 7,69E-02 7,78E-01 MNR 0 7,53E-03 0 7,26E-02 -4,19E-01
TPE
Total use of renewable primary energy resources (RPEE+RPEM)
MJ 2,10E+01 1,38E+00 6,57E-01 MNR 0 1,35E-01 0 5,40E-01 -2,15E+00
NRPE Non renewable primary energy used as Energy carrier, e.g. energy from fossil fuel power plants or
transportation
MJ 9,92E-01 0,00E+00 -2,98E-02 MNR 0 0,00E+00 0 0,00E+00 0,00E+00
NRPM Non renewable primary energy resources used as raw materials, e.g. oil derivatives used as feedstock material
for the petrochemical industry / plastics
MJ 2,20E+01 1,38E+00 6,27E-01 MNR 0 1,35E-01 0 5,40E-01 -2,15E+00
TRPE
Total use of non renewable primary energy resources (NRPE+NRPM)
kg 5,17E-02 0,00E+00 1,03E-03 MNR 0 0,00E+00 0 0,00E+00 1,92E-01
SM
Secondary materials, Use of recycled material, e.g. return wool
MJ 0,00E+00 0,00E+00 0,00E+00 MNR 0 0,00E+00 0 0,00E+00 0,00E+00
RSF Renewable secondary fuels. E.g. used frying oil. Renewable secondary fuels can represent a limited resource why
increased consumption potentially can create shortages.
MJ 0,00E+00 0,00E+00 0,00E+00 MNR 0 0,00E+00 0 0,00E+00 0,00E+00
NRSF
Non-renewable secondary fuels, e.g. waste oil
m3 6,68E-03 8,80E-05 5,63E-04 MNR 0 8,62E-06 0 1,33E-04 -7,63E-04
W net fresh water consumption. Fresh water is a limited resource why high consumption of fresh water can create
local shortages
RPEE Renewable primary energy resources used as energy carrier; RPEM Renewable primary energy
resources used as raw materials; TPE Total use of renewable primary energy resources; NRPE Non
renewable primary energy resources used as energy carrier; NRPM Non renewable primary energy
resources used as materials; TRPE Total use of non renewable primary energy resources; SM Use of
secondary materials; RSF Use of renewable secondary fuels; NRSF Use of non renewable secondary fuels; W
Use of net fresh water
EPD for the best environmental decision 13
End of life – Waste
Parameter Unit A1-3 A4 A5 B1-B7 C1 C2 C3 C4 D
kg 6,46E-07 6,93E-11 8,71E-09 MNR 0 6,81E-12 0 5,73E-11 -9,85E-10
HW
Hazardous waste, collected and sent special treatment
kg 4,70E-02 2,05E-04 4,66E-02 MNR 0 2,01E-05 0 2,69E+00 -2,05E-02
NHW Non Hazardous Waste Disposed consists of inactive (inert) waste e.g. construction waste that typically is sent to
landfill. An increased fraction is sent to reuse or recycling.
kg 1,01E-04 1,67E-06 1,71E-05 MNR 0 1,63E-07 0 5,64E-06 -1,46E-05
RW
Radioactive Waste Disposed. Mainly represents waste from nuclear power plants.
HW Hazardous waste disposed; NHW Non hazardous waste disposed; RW Radioactive waste disposed
End of life – output flow
Parameter Unit A1-3 A4 A5 B1-B7 C1 C2 C3 C4 D
kg 0,00E+00 0,00E+00 0,00E+00 MNR 0 0,00E+00 0 0,00E+00 0,00E+00
CR
Components for Re-Use. Materials or components which are re-used outside the system boundary.
kg 0,00E+00 0,00E+00 3,19E-02 MNR 0 0,00E+00 0 0,00E+00 0,00E+00
MR
Materials for Recycling. Materials recycled outside the system boundary
kg 0,00E+00 0,00E+00 5,41E-02 MNR 0 0,00E+00 0 0,00E+00 0,00E+00
MER Materials for Energy Recovery. Materials utilised in power plants as secondary fuels outside the system
boundary
kg 0,00E+00 0,00E+00 1,79E-01 MNR 0 0,00E+00 0 0,00E+00 0,00E+00
EEE
Exported electrical energy: Electrical energy from incineration of waste or landfill gas
kg 0,00E+00 0,00E+00 5,37E-01 MNR 0 0,00E+00 0 0,00E+00 0,00E+00
ETE
Exported thermal energy. Thermal energy, e.g. steam from incineration of waste or landfill gas
CR Components for reuse; MR Materials for recycling; MER Materials for energy recovery; EEE Exported
electric energy; ETE Exported thermal energy
Information describing the biogenic carbon content at the factory gate
Biogenic carbon content Unit Value
Biogenic carbon content in product kg C 0
Biogenic carbon content in the accompanying packaging kg C 0,0481
EPD for the best environmental decision 14
GWP-total interpretation
Benefits
End of & Loads
Global
Product Construction stage Use life beyond
Warming
stage stage stage Total system
Potential-total A1-A3 A4 A5 B1-B7 C1-C4 A1-C4 D
2.03
2,41
0.23
0.10 0.05
Kg CO2 eqv./FU
-0.08
The main GWP contribution from the product life cycle is linked to the Product stage (A1-A3).
This is primarily related to the materials delivered to the factory gate and consumption of
electricity and coke.
The energy consumption linked to A3, is calculated and verified externally as 100% renewable
electricity from Danish windpower and 100% Danish biogas and the coke (consumed on
conventional line). The investment in low carbon energy sources secures a significantly lower
GWP-total (A1-C4) as compared to conventional energy sources (up to 50%), for the TOPROCK
system specific the reduction is approximately 25%.
The CO absorbed by the wood in the wooden pallets is represented by a negative GWP-
2
biogenic. This reduces the GWP-total (A1-A3) by approximately11%.
The GWP-Biogenic, ie the carbon stored in the wooden pallets, is released during the
construction stage phase (A5) where the wood is presumed incinerated with energy recovery.
The benefits from energy recovery (a negative GWP) from incineration of packaging materials
(wood pallets and plastic foils) is allocated to Benefits & Loads beyond system (D).
Approximately 50% of the GWP-total from the assembly phase (A5) is linked to fosssil
emissions from incineration of plactic foils and handling of surplus stone wool/installation
waste (2%).
EPD for the best environmental decision 15
Impacts linked to end of life stages (C1-C4) are primarily linked to transportation of stone wool
to recycling or to landfill.
Melting virgin materials or re-melting returned ROCKWOOL stone wool are both similarly
energy intensive processes. Increasing the recycling rate for return wool, will therefore not lead
to great variations in the overall GWP profile. However, increased recycling will be linked
directly to reduction of waste sent to landfill.
Additional Norwegian requirements
Greenhouse gas emission from the use of electricity in the manufacturing phase
The calculations of applied electricity and gas for the manufacturing process (A3) are made
taking into account 100% renewable electricity from Danish wind power and 100% Danish
biogas use. The renewable sources of energy and electricity are evidenced by Guarantee of
Origin certificates (GOs).
National production mix from import, low voltage (production of transmission lines, in addition
to direct emissions and losses in grid) for wind power electricity production.
National electricity grid (with GOs) Unit Value
Denmark, Wind power, GaBi version 10.0.1 (2021) kg CO2 -eq/kWh 0,006
Additional GWP results calculations using the physical national electricity grid mix and
gas mix (energy sources without a guarantees of origins)
National electricity grid Unit Value
Denmark, GaBi version 10.0.1 (2021) kg CO2 -eq/kWh 0,240
Indicator Unit A1-3
GWP-total kg CO2 eq. 2,66E+00
GWP-fossil kg CO2 eq. 2,82E+00
GWP-biogenic kg CO2 eq. -1,62E-01
GWP-LULUC kg CO2 eq. 1,39E-03
The complete additional results for all the impact categories representing the calculations
without guarantees of origins, applying Danish national production mix for electricity and
natural gas for gas are given in Appendix: Additional LCA Results without GOs.
Additional environmental impact indicators required in NPCR Part A for construction
products
In order to increase the transparency of biogenic carbon contribution to climate impact, the
indicator for GWP has been sub-divided into the following:
GWP-IOBC Climate impacts calculated according to the principle of instantaneous oxidation
GWP-BC Climate impacts from the net uptake and emission of biogenic carbon from each
module.
EPD for the best environmental decision 16
In addition, EP-freshwater shall also declared as PO4 eq.
Indicator Unit A1-3 A4 A5 B C1 C2 C3 C4 D
EP- kg PO4
2,76E-03 7,04E-05 7,65E-05 MNR 0 1,11E-06 0 1,70E-05 -1,62E-05
freshwater* eq.
kg CO2
GWP-IOBC 2,19E+00 7,40E-02 6,26E-02 MNR 0 1,02E-02 0 4,07E-02 -8,79E-02
eq.
kg CO2
GWP-BC -1,64E-01 0,00E+00 1,65E-01 MNR 0 0,00E+00 0 0,00E+00 8,78E-03
eq.
kg CO2
GWP 2,03E+00 7,40E-02 2,28E-01 MNR 0 1,02E-02 0 4,07E-02 -7,92E-02
eq.
EP-freshwater* Eutrophication potential, fraction of nutrients reaching freshwater end compartment.
Declared as PO4 eq. GWP-IOBC Global warming potential calculated according to the principle of
instantaneous oxidation. GWP-BC Global warming potential from net uptake and emissions of biogenic
carbon from the materials in each module. GWP Global warming potential
Hazardous substances
The declaration is based upon reference to threshold values and/or test results and/or material
safety data sheets provided to EPD verifiers. Documentation available upon request to EPD
owner.
□ The product contains no substances given by the REACH Candidate list or the Norwegian
priority list.
□ The product contains substances given by the REACH Candidate list or the Norwegian
priority list that are less than 0,1 % by weight.
□ The product contain dangerous substances, more then 0,1% by weight, given by the
REACH Candidate List or the Norwegian Priority list, see table.
□ The product contains no substances given by the REACH Candidate list or the Norwegian
priority list. The product is classified as hazardous waste (Avfallsforskiften, Annex III),
see table.
Mineral wool fibers produced by ROCKWOOL are classified as non-hazardous under REACH
(Regulation (EC) No 1272/2008 of the European Parliament and of the Council Cof 16
December 2008 on classification, labelling and packaging of substances and mixtures).
ROCKWOOL® are registered with REACH under the following definition: “Man-made vitreous
(silicate) fibers with random orientation with alkaline oxide and alkali earth
oxide(Na2O+K2O+CaO+MgO+BaO) content greater than 18% by weight and fulfilling one of the
Note Q conditions”. ROCKWOOL products produced in Europe fulfil the Note Q requirements.
This is certified by the independent certification body EUCEB (European Certification Board for
mineral wool products). More information on EUCEB can be found at www.euceb.org.
Indoor environment
There are no legal requirements for indoor emissions of stone wool thermal insulation
products.
Carbon footprint
Carbon footprint of 1 m2 of a 39 mm thick ROCKWOOL® TOPROCK System with a density of 75
kg/m3 (R=1m2K/W) is 2,41 kg CO2 eq (including Module A1-C4). This is elaborated per module
in the results section.
EPD for the best environmental decision 17
APPENDIX: Additional LCA Results without GOs
The LCA Results were calculated additionally without taking into account the purchase of
guarantees of origin. Based on these results the contribution of green electricity and biogas to
the reduction of environmental impacts can be observed. ROCKWOOL Nordics has committed
to continious purchase of renewable energy certificates for at least the validity period of this
declaration.
Calculations are done applying Danish national production mix for electricity and natural gas
for gas in manufacturing processes (A3).
National electricity grid Unit Value
Denmark, GaBi version 10.0.1 (2021) kg CO2 -eq/kWh 0,240
Core environmental impact indicators
Indicator Unit A1-3 A4 A5 B C1 C2 C3 C4 D
GWP-total kg CO2 eq. 2,66E+00 1,04E-01 2,00E-01 MNR 0 1,02E-02 0 4,07E-02 -7,91E-02
GWP-fossil kg CO2 eq. 2,82E+00 1,03E-01 3,67E-02 MNR 0 1,01E-02 0 4,06E-02 -8,79E-02
0,00E+0 0,00E+0
GWP-biogenic kg CO2 eq.
-1,62E-01 0,00E+00 1,63E-01 MNR 0 0 0 0 8,78E-03
GWP-LULUC kg CO2 eq. 1,39E-03 8,47E-04 2,74E-05 MNR 0 8,31E-05 0 1,19E-04 -2,99E-05
kg CFC11
ODP
eq. 6,81E-09 1,32E-17 3,22E-10 MNR 0 1,29E-18 0 1,58E-16 -6,92E-15
AP mol H⁺ eq. 2,50E-02 9,18E-05 5,53E-04 MNR 0 1,06E-05 0 2,90E-04 -2,27E-04
EP-freshwater kg P eq. 1,54E-05 1,89E-06 4,62E-07 MNR 0 3,01E-08 0 6,81E-08 -9,79E-08
EP-marine kg N eq. 2,99E-03 2,70E-05 7,97E-05 MNR 0 3,51E-06 0 7,52E-05 -4,95E-05
EP-terrestial mol N eq. 9,43E-02 3,28E-04 2,08E-03 MNR 0 4,16E-05 0 8,24E-04 -5,39E-04
kg NMVOC
POCP
eq. 6,48E-03 7,80E-05 1,77E-04 MNR 0 9,31E-06 0 2,27E-04 -1,55E-04
ADP-M&M kg Sb eq. 5,03E-07 7,86E-09 1,18E-08 MNR 0 7,72E-10 0 3,83E-09 -1,46E-08
ADP-fossil MJ 3,21E+01 1,38E+00 8,52E-01 MNR 0 1,35E-01 0 5,40E-01 -2,07E+00
WDP m³ 2,38E-01 8,96E-04 2,23E-02 MNR 0 8,81E-05 0 4,36E-03 -2,76E-02
GWP-total: Global Warming Potential; GWP-fossil: Global Warming Potential fossil fuels; GWP-biogenic:
Global Warming Potential biogenic; GWP-LULUC: Global Warming Potential land use and land use change;
ODP: Depletion potential of the stratospheric ozone layer; AP: Acidification potential, Accumulated
Exceedance; EP-freshwater: Eutrophication potential, fraction of nutrients reaching freshwater end
compartment; See “additional Norwegian requirements” for indicator given as PO4 eq. EP-marine:
Eutrophication potential, fraction of nutrients reaching freshwater end compartment; EP-terrestial:
Eutrophication potential, Accumulated Exceedance; POCP: Formation potential of tropospheric ozone; ADP-
M&M: Abiotic depletion potential for non-fossil resources (minerals and metals); ADP-fossil: Abiotic
depletion potential for fossil resources; WDP: Water deprivation potential, deprivation weighted water
counsumption
Reading example: 9,0 E-03 = 9,0*10-3 = 0,009
EPD for the best environmental decision 18
Additional environmental impact indicators
Indicator Unit A1-3 A4 A5 B C1 C2 C3 C4 D
Disease
PM 2,03E-07 5,82E-10 4,46E-09 MNR 0 6,13E-11 0 3,59E-09 -3,41E-09
incid.
kBq
IRP 4,75E-02 2,39E-04 3,05E-03 MNR 0 2,34E-05 0 5,94E-04 -1,67E-03
U235 eq.
ETP-fw CTUe 7,35E+00 9,94E-01 2,44E-01 MNR 0 9,76E-02 0 3,07E-01 -8,87E-02
HTP-c CTUh 2,33E-09 2,01E-11 5,20E-11 MNR 0 1,97E-12 0 4,53E-11 -1,10E-11
HTP-nc CTUh 1,82E-08 1,03E-09 8,04E-10 MNR 0 1,02E-10 0 4,99E-09 -4,41E-10
Dimensi
SQP 3,58E+01 4,73E-01 7,53E-01 MNR 0 4,63E-02 0 1,09E-01 -1,80E+00
onless
PM: Particulate matter emissions; IRP: Ionising radiation, human health; ETP-fw: Ecotoxicity (freshwater);
ETP-c: Human toxicity, cancer effects; HTP-nc: Human toxicity, non-cancer effects; SQP: Land use related
impacts / soil quality
Classification of disclaimers to the declaration of core and additional environmental
impact indicators
ILCD classification Indicator Disclaimer
Global warming potential (GWP) None
ILCD type / level 1 Depletion potential of the stratospheric ozone layer (ODP) None
Potential incidence of disease due to PM emissions (PM) None
Acidification potential, Accumulated Exceedance (AP) None
Eutrophication potential, Fraction of nutrients reaching freshwater end
None
compartment (EP-freshwater)
Eutrophication potential, Fraction of nutrients reaching marine end
None
ILCD type / level 2 compartment (EP-marine)
Eutrophication potential, Accumulated Exceedance (EP-terrestrial) None
Formation potential of tropospheric ozone (POCP) None
Potential Human exposure efficiency relative to U235 (IRP) 1
Abiotic depletion potential for non-fossil resources (ADP-
2
minerals&metals)
Abiotic depletion potential for fossil resources (ADP-fossil) 2
Water (user) deprivation potential, deprivation-weighted water
2
consumption (WDP)
ILCD type / level 3 Potential Comparative Toxic Unit for ecosystems (ETP-fw) 2
Potential Comparative Toxic Unit for humans (HTP-c) 2
Potential Comparative Toxic Unit for humans (HTP-nc) 2
Potential Soil quality index (SQP) 2
Disclaimer 1 – This impact category deals mainly with the eventual impact of low dose ionizing radiation on
human health of the nuclear fuel cycle. It does not consider effects due to possible nuclear accidents, occupational
exposure nor due to radioactive waste disposal in underground facilities. Potential ionizing radiation from the soil,
from radon and from some construction materials is also not measured by this indicator.
Disclaimer 2 – The results of this environmental impact indicator shall be used with care as the uncertainties on
these results are high or as there is limited experienced with the indicator
EPD for the best environmental decision 19
Resource use
Indicator Unit A1-3 A4 A5 B C1 C2 C3 C4 D
RPEE MJ 5,99E+00 7,69E-02 9,51E-02 MNR 0 7,53E-03 0 7,26E-02 -4,19E-01
RPEM MJ 1,91E+00 0,00E+00 -5,74E-02 MNR 0 0,00E+00 0 0,00E+00 0,00E+00
TPE MJ 7,90E+00 7,69E-02 3,77E-02 MNR 0 7,53E-03 0 7,26E-02 -4,19E-01
NRPE MJ 3,18E+01 1,38E+00 1,93E-01 MNR 0 1,35E-01 0 5,40E-01 -2,15E+00
NRPM MJ 9,92E-01 0,00E+00 -2,98E-02 MNR 0 0,00E+00 0 0,00E+00 0,00E+00
TRPE MJ 3,27E+01 1,38E+00 1,66E-01 MNR 0 1,35E-01 0 5,40E-01 -2,15E+00
SM kg 5,17E-02 0,00E+00 0,00E+00 MNR 0 0,00E+00 0 0,00E+00 -1,92E-01
RSF MJ 0,00E+00 0,00E+00 0,00E+00 MNR 0 0,00E+00 0 0,00E+00 0,00E+00
NRSF MJ 0,00E+00 0,00E+00 0,00E+00 MNR 0 0,00E+00 0 0,00E+00 0,00E+00
W m3 8,26E-03 8,80E-05 4,25E-04 MNR 0 8,62E-06 0 1,33E-04 -7,63E-04
RPEE Renewable primary energy resources used as energy carrier; RPEM Renewable primary energy
resources used as raw materials; TPE Total use of renewable primary energy resources; NRPE Non
renewable primary energy resources used as energy carrier; NRPM Non renewable primary energy
resources used as materials; TRPE Total use of non renewable primary energy resources; SM Use of
secondary materials; RSF Use of renewable secondary fuels; NRSF Use of non renewable secondary fuels; W
Use of net fresh water
End of life – Waste
Indicator Unit A1-3 A4 A5 B C1 C2 C3 C4 D
HW kg 6,53E-07 6,93E-11 1,31E-08 MNR 0 6,81E-12 0 5,73E-11 -9,85E-10
NHW kg 5,75E-02 2,05E-04 4,67E-02 MNR 0 2,01E-05 0 2,69E+00 -2,05E-02
RW kg 3,47E-04 1,67E-06 1,99E-05 MNR 0 1,63E-07 0 5,64E-06 -1,46E-05
HW Hazardous waste disposed; NHW Non hazardous waste disposed; RW Radioactive waste disposed
End of life – output flow
Indicator Unit A1-3 A4 A5 B C1 C2 C3 C4 D
CR kg 0,00E+00 0,00E+00 0,00E+00 MNR 0 0,00E+00 0 0,00E+00 0,00E+00
MR kg 0,00E+00 0,00E+00 3,19E-02 MNR 0 0,00E+00 0 0,00E+00 0,00E+00
MER kg 0,00E+00 0,00E+00 0,00E+00 MNR 0 0,00E+00 0 0,00E+00 0,00E+00
EEE MJ 0,00E+00 0,00E+00 1,79E-01 MNR 0 0,00E+00 0 0,00E+00 0,00E+00
ETE MJ 0,00E+00 0,00E+00 5,37E-01 MNR 0 0,00E+00 0 0,00E+00 0,00E+00
CR Components for reuse; MR Materials for recycling; MER Materials for energy recovery; EEE Exported
electric energy; ETE Exported thermal energy
EPD for the best environmental decision 20
Bibliography
ISO 14025:2010 Environmental labels and declarations - Type III environmental
declarations - Principles and procedures
ISO 14044:2006 Environmental management - Life cycle assessment -
Requirements and guidelines
EN 15804:2012+A2:2019 Sustainability of construction works - Environmental product
declaration - Core rules for the product category of construction
products
EN 12939:2000 Thermal performance of building materials and products -
Determination of thermal resistance by means of guarded hot
plate and heat flow meter methods - Thick products of high and
medium thermal resistance
EN 12667:2001 Thermal performance of building materials and products –
determination of thermal resistance by means of guarded hot
plate and heat flow meter methods – Products of high and
medium thermal resistance
EN 13501-1:2007+A1:2009 Fire classification of construction products and building elements
-Part 1: Classification using data from reaction to fire tests
ISO 21930:2007 Sustainability in building construction - Environmental
declaration of building products
PCR NPCR Part A Construction products and services
PCR NPCR 012:2018 version 2. Part B for Thermal insulation products
Larisa Xanthopoulou Background LCA report for EPDs ROCKWOOL Nordics, Feb. 2022
Larisa Xanthopoulou ROCKWOOL Rules for publishing EPDs, ver.3, December 2021
Program Operator tlf +47 23 08 80 00
The Norwegian EPD Foundation
Post Box 5250 Majorstuen, 0303 Oslo e-post: post@epd-norge.no
Norway web www.epd-norge.no
Publisher tlf +47 23 08 80 00
The Norwegian EPD Foundation
Post Box 5250 Majorstuen, 0303 Oslo e-post: post@epd-norge.no
Norway web www.epd-norge.no
Owner of the decleration tlf +45 46 56 16 16
ROCKWOOL Nordics (ROCKWOOL Group)
Hovedgaden 501, 2640 Hedehusene, e-post: christian.kofod@rockwool.com
Denmark web www.rockwool.com/dk
Author of the life cycle assesment tlf +45 46 56 03 00
Larisa Xanthopoulou Fax
ROCKWOOL International A/S e-post: info@rockwool.com
Hovedgaden 584, 2640 Hedehusene,
web www.rockwool.com
Denmark
EPD for the best environmental decision 21
EPD for the best
environmental
decision
The Norwegian EPD foundation
www.epd-norge.no
