ENVIRONMENTAL PRODUCT DECLARATION
as per ISO 14025 and EN 15804+A2
Owner of the Declaration European Association for Panels and Profiles e. V. (PPA-Europe)
Publisher Institut Bauen und Umwelt e.V. (IBU)
Programme holder Institut Bauen und Umwelt e.V. (IBU)
Declaration number EPD-PPA-20240128-CBG2-EN
Issue date 19.07.2024
Valid to 18.07.2029
Double skin steel faced sandwich panels with a core made of
polyurethane
PPA-Europe
www.ibu-epd.com | https://epd-online.com
General Information
PPA-Europe Double skin steel faced sandwich panels with a
core made of polyurethane
Programme holder Owner of the declaration
IBU – Institut Bauen und Umwelt e.V. European Association for Panels and Profiles e. V. (PPA-Europe)
Hegelplatz 1 Europark Fichtenhain A 13a
10117 Berlin 47807 Krefeld
Germany Germany
Declaration number Declared product / declared unit
EPD-PPA-20240128-CBG2-EN 1 m² prefabricated double skin steel faced sandwich panels with an
insulating core made of polyurethane rigid foam
This declaration is based on the product category rules: Scope:
Double skin metal faced sandwich panels, 01.08.2021 This document is an association EPD for 1 m² of PU Core sandwich panel
(PCR checked and approved by the SVR) with 100 mm thickness and it represents an average EPD, based on
vertical averaging of the specific producer datasets under consideration of
the yearly productionamounts. Its applicability is limited to continuously
Issue date produced double skin steel faced sandwich panels with an insulating core
made of polyurethane, which are manufactured by member companies of
19.07.2024
the European Association for Panels and Profiles.
The following member companies of the European Association for Panels
Valid to
and Profiles have provided data for the year 2022:
18.07.2029
1. ArcelorMittal Group, Construction Division
• ArcelorMittal Construction Austria
• ArcelorMittal Construction Belgium
• ArcelorMittal Construction Deutschland
• ArcelorMittal Construcción España
• ArcelorMittal Construction France
• Arcelormittal Construction Polska
• ArcelorMittal Construção Portugal
• Europerfil
• Pflaum & Söhne Bausysteme
2. Assan Panel Sanayi ve Ticaret
Dipl.-Ing. Hans Peters 3. Brucha
(Chairman of Institut Bauen und Umwelt e.V.) 4. Fischer Profil
5. Huurre Iberica
6. ISOCAB France (Kingspan Group)
7. Isolpack
8. Joris Ide Belgium (Joris Ide Group)
9. Metecno Bausysteme
10. Montana Bausysteme
11. PAGOUNI
12. SAB-profiel
These companies are representative for the European production of steel
faced sandwich panels with polyurethane core.
This EPD comprises an annex with LCA results for two additional sandwich
panel thicknesses: 40 mm and 160 mm. Additionally, the EPD annex
contains LCA results for 1 kg steel sheet used for the panel faces and 1 m³
polyurethane (PU) used for the panel core, which allows the combination
and estimation of LCA results for different panel variations.
The owner of the declaration shall be liable for the underlying information
and evidence; the IBU shall not be liable with respect to manufacturer
information, life cycle assessment data and evidences.
The EPD was created according to the specifications of EN 15804+A2. In
the following, the standard will be simplified as EN 15804.
Verification
The standard EN 15804 serves as the core PCR
Independent verification of the declaration and data according to ISO
14025:2011
internally X externally
1 Environmental Product Declaration - PPA-Europe - Double skin steel faced sandwich panels with a core made of polyurethane
Florian Pronold Mr Olivier Muller,
(Managing Director Institut Bauen und Umwelt e.V.) (Independent verifier)
2 Environmental Product Declaration - PPA-Europe - Double skin steel faced sandwich panels with a core made of polyurethane
Product
characteristics according to EN 14509
Product description/Product definition
The EPD applies to prefabricated double-skin steel faced
sandwich panels with a core made of polyurethane, which are Base materials/Ancillary materials
produced by member companies of PPA-Europe.
Composition of the sandwich panels:
The profiled internal and external faces are made of a core of
steel, which is protected against corrosion with zinc and organic
coatings. The thermal insulating core is made of polyurethane
rigid foam according to /EN 13165/ with sealing tapes. The core
is bonded to the steel sheets on both sides, to ensure a certain
resistance to shear forces of the panel.
The LCA is based on vertical averaging of the specific producer
datasets under consideration of the respective yearly
production amounts. For the placing of the product on the
market in the European Union/European Free Trade
Association (EU/EFTA) (with the exception of Switzerland), Steel sheet according to EN 10346:
/CPR/ applies. The product needs a Declaration of S280 GD to S350 GD
Performance taking into consideration /EN 14509/ and the CE-
marking. The data listed in the respective Declaration of Metallic coating according to EN 10346:
Performance apply. Zinc Z275, coating 275 g/m²
For the application and use, the respective national provisions The zinc layer has a content of at least 99 weight percent zinc
apply. and a typical thickness of 20 μm.
Application Organic coating according to EN 10169:
The products are used for self-supporting and structural Polyester (SP), coil coating, 25 μm on the application side and
applications in roof, wall and ceiling structures. max. 15 μm on the backside.
Sandwich panels in wall and roof applications take on tasks of Thermal insulation core according to EN 13165:
the building physics, especially sound, heat and moisture Rigid polyurethane foam mainly made of isocyanate and polyol
safety. They simultaneously perform the function of air tightness
of the building envelope. The panels contain sealing tapes (amount on total weight < 0,6
%).
Technical Data
Technical specifications for sandwich panels with a core made The product does not contain any SVHCs (Substances of Very
of polyurethane are: High Concern) REACH.
• /EN 14509/
Reference service life
• /EN 13165/
Double-skin steel faced sandwich panels used in lightweight
Constructional Data
metal constructions must withstand a term of protection of at
Name Value Unit least 15 years. The term of protection is the period until first
36 - slight renewals in the surface are required, only if there is no
Density of the insulation kg/m3
43 need of frequent inspections and service.
Thickness of the element , when the outer layers
are flat, this is the overall height of the element The term of protection depends on the location, weather
(D); on heavily profiled elements, this is the 100 mm conditions and the quality of the coating.
continuous core thickness without profile (dc)
Double-skin steel faced sandwich panels exhibit an estimated
Thickness of the inner layer 0.5 mm
service life of 50 years depending on the use conditions.
Weight 12.6 kg/m²
Thickness of the outer layer 0.6 mm The information in this section does not refer to a reference
Performance data of the product in accordance with the service life according to ISO 15686.
declaration of performance with respect to its essential
LCA: Calculation rules
Name Value Unit
Declared Unit
Declared unit 1 m2
The declared unit is 1 m² of sandwich panel. The averaging is
done based on the yearly production volume per company. Surface weight of the panel (total value) 12.6 kg/m²
Conversion factor to 1 kg 0.079 -
Declared unit
Conversion factor is 1/12.6
System boundary
3 Environmental Product Declaration - PPA-Europe - Double skin steel faced sandwich panels with a core made of polyurethane
Type of the EPD: cradle to gate - with options, module C1-C4
and module D (A1-A3, C, D and additional modules A4 and A5). For the end of life, it is assumed that the steel proportion is
recycled with benefits for the recycling potential declared in
Production stage (modules A1-A3) includes processes that module D and the PU proportion is incinerated (module C3)
provide materials and energy input for the system, with benefits given for energy substitution in module D.
manufacturing and transport processes up to the factory gate,
as well as waste processing. Geographic Representativeness
Module A4: Delivery to the construction site with a transport Land or region, in which the declared product system is
distance of 100 km. manufactured, used or handled at the end of the product´s
Module A5: Disposal of transport packaging at the construction lifespan: Europe
site and energy for installation.
Comparability
Module C1: Dismantling with the use of machinery (diesel
Basically, a comparison or an evaluation of EPD data is only
driven).
possible if all the data sets to be compared were created
Module C2: Transport to the site of end-of-life treatment-
according to EN 15804 and the building context, respectively
transport distance of 50 km.
the product-specific characteristics of performance, are taken
Module C3: Metal recycling of the steel sheets and incineration
into account. LCA FE (fka GaBi) software and databases
of the PU core material with energy recovery.
Sphera LCA FE were used as calculation basis.
Module D: Potential benefits for substitution processes or
recycling materials from modules A5 and C3.
LCA: Scenarios and additional technical information
polystyrene, polyethylene foil, cardboard and wooden pallets.
Characteristic product properties of biogenic carbon A5 covers the treatment of packaging material at the point of
Information on describing the biogenic Carbon Content at installation.
factory gate
Name ValueUnit Installation into the building (A5)
Biogenic carbon content in accompanying kg Name Value Unit
0.042
packaging C Output substances following waste treatment on
0.185 kg
site
Note: 1 kg of biogenic carbon is equivalent to 44/12 kg of CO
2
Machineries for installation - diesel driven 0.233kg/m²
Note: 1 kg of biogenic carbon is equivalent to 44/12 kg of CO .
2 End of life (C1-C4)
Name Value Unit
The following technical information is a basis for the declared Machineries for dismantling - diesel driven 0.233 kg/m²
modules. Collected separately waste type 12.6 kg
Recycling 7.89 kg
Transport to the building site (A4) Energy recovery 4.05 kg
Name Value Unit Landfilling - kg
Transport distance 100 km Reuse, recovery or recycling potential (D)
Capacity utilisation (including empty runs) 61 % Resulting potential benefits and loads for the metal recycling as
well as the thermal treatment of PU are declared in module D.
Installation (A5)
The following packaging material is considered in A1-A3:
4 Environmental Product Declaration - PPA-Europe - Double skin steel faced sandwich panels with a core made of polyurethane
LCA: Results
DESCRIPTION OF THE SYSTEM BOUNDARY (X = INCLUDED IN LCA; MND = MODULE OR INDICATOR NOT DECLARED; MNR
= MODULE NOT RELEVANT)
Benefits and
Construction loads beyond
Product stage Use stage End of life stage
process stage the system
boundaries
la ire ta m w a Ry lp p u s tro p s n a rT g n iru tc a fu n a M e h t m o rf tro p s n a rTe tis e h t o t e ta g y lb m e s s A e s U e c n a n e tn ia M ria p e R tn e m e c a lp e R tn e m h s ib ru fe R y g re n e la n o ita re p Oe s u re ta w la n o ita re p Oe s u n o itc u rts n o c -e Dn o itilo m e d tro p s n a rT g n is s e c o rp e ts a W la s o p s iD -e s u e R-y re v o c e R-g n ilc y c e Rla itn e to p
A1 A2 A3 A4 A5 B1 B2 B3 B4 B5 B6 B7 C1 C2 C3 C4 D
X X X X X MND MND MNR MNR MNR MND MND X X X X X
RESULTS OF THE LCA - ENVIRONMENTAL IMPACT according to EN 15804+A2: 1 m² PU sandwich panel 100 mm (12.6 kg/m²)
Parameter Unit A1-A3 A4 A5 C1 C2 C3 C4 D
GWP-total kg CO 2 eq 3.41E+01 9.11E-02 7.17E-02 8.26E-01 4.55E-02 8.92E+00 0 -1.49E+01
GWP-fossil kg CO 2 eq 3.4E+01 9E-02 3.43E-02 8.15E-01 4.5E-02 8.92E+00 0 -1.49E+01
GWP-biogenic kg CO 2 eq 4.37E-02 2.66E-04 3.74E-02 3.21E-03 1.33E-04 6.39E-04 0 9.05E-03
GWP-luluc kg CO 2 eq 1.64E-02 8.34E-04 -6.73E-07 7.53E-03 4.17E-04 1.43E-05 0 -6.45E-03
ODP kg CFC11 eq 2.3E-11 1.17E-14 2.83E-14 1.06E-13 5.86E-15 7.2E-13 0 1.9E-11
AP mol H+ eq 1.3E-01 1.16E-04 3.92E-05 4.77E-03 5.78E-05 5.26E-03 0 -3.05E-02
EP-freshwater kg P eq 6.74E-05 3.29E-07 8.09E-09 2.97E-06 1.65E-07 1.95E-07 0 -5.75E-06
EP-marine kg N eq 3.23E-02 3.92E-05 1.51E-05 2.33E-03 1.96E-05 2.55E-03 0 -8.05E-03
EP-terrestrial mol N eq 3.48E-01 4.71E-04 1.91E-04 2.58E-02 2.36E-04 2.93E-02 0 -8.98E-02
kg NMVOC
POCP 1E-01 9.96E-05 3.88E-05 6.19E-03 4.98E-05 6.54E-03 0 -2.51E-02
eq
ADPE kg Sb eq 5.46E-04 5.93E-09 4.69E-11 5.36E-08 2.96E-09 6.86E-09 0 8.78E-06
ADPF MJ 5.3E+02 1.23E+00 3.91E-02 1.11E+01 6.13E-01 2.36E+00 0 -1.4E+02
m3 world eq
WDP 2.09E+00 1.09E-03 1.22E-02 9.83E-03 5.44E-04 8.78E-01 0 1.56E-01
deprived
GWP = Global warming potential; ODP = Depletion potential of the stratospheric ozone layer; AP = Acidification potential of land and water; EP =
Eutrophication potential; POCP = Formation potential of tropospheric ozone photochemical oxidants; ADPE = Abiotic depletion potential for non-fossil
resources; ADPF = Abiotic depletion potential for fossil resources; WDP = Water (user) deprivation potential)
RESULTS OF THE LCA - INDICATORS TO DESCRIBE RESOURCE USE according to EN 15804+A2: 1 m² PU sandwich panel
100 mm (12.6 kg/m²)
Parameter Unit A1-A3 A4 A5 C1 C2 C3 C4 D
PERE MJ 3.17E+01 8.92E-02 1.54E+00 8.06E-01 4.46E-02 4.8E-01 0 -8.83E-01
PERM MJ 1.56E+00 0 -1.53E+00 0 0 -3.6E-02 0 0
PERT MJ 3.33E+01 8.92E-02 1.32E-02 8.06E-01 4.46E-02 4.44E-01 0 -8.83E-01
PENRE MJ 4.26E+02 1.23E+00 3.27E+00 1.11E+01 6.15E-01 1.04E+02 0 -1.41E+02
PENRM MJ 1.05E+02 0 -3.23E+00 0 0 -1.02E+02 0 0
PENRT MJ 5.32E+02 1.23E+00 3.9E-02 1.11E+01 6.15E-01 2.36E+00 0 -1.41E+02
SM kg 2.13E+00 0 0 0 0 0 0 0
RSF MJ 0 0 0 0 0 0 0 0
NRSF MJ 0 0 0 0 0 0 0 0
FW m3 9.27E-02 9.77E-05 2.86E-04 8.83E-04 4.89E-05 2.07E-02 0 -8.54E-03
PERE = Use of renewable primary energy excluding renewable primary energy resources used as raw materials; PERM = Use of renewable primary
energy resources used as raw materials; PERT = Total use of renewable primary energy resources; PENRE = Use of non-renewable primary energy
excluding non-renewable primary energy resources used as raw materials; PENRM = Use of non-renewable primary energy resources used as raw
materials; PENRT = Total use of non-renewable primary energy resources; SM = Use of secondary material; RSF = Use of renewable secondary fuels;
NRSF = Use of non-renewable secondary fuels; FW = Use of net fresh water
RESULTS OF THE LCA – WASTE CATEGORIES AND OUTPUT FLOWS according to EN 15804+A2:
1 m² PU sandwich panel 100 mm (12.6 kg/m²)
Parameter Unit A1-A3 A4 A5 C1 C2 C3 C4 D
HWD kg 7.09E-06 3.81E-12 4.14E-13 3.44E-11 1.91E-12 2.08E-10 0 -3.29E-09
NHWD kg 1.15E+00 1.88E-04 4.63E-03 1.7E-03 9.38E-05 4.49E-02 0 -3.69E-01
RWD kg 6.69E-03 2.3E-06 1.38E-06 2.08E-05 1.15E-06 9.67E-05 0 -2.71E-03
CRU kg 0 0 0 0 0 0 0 0
MFR kg 1.11E-01 0 0 0 0 7.89E+00 0 0
MER kg 0 0 0 0 0 0 0 0
EEE MJ 0 0 9.01E-02 0 0 1.54E+01 0 0
EET MJ 0 0 2.12E-01 0 0 2.76E+01 0 0
5 Environmental Product Declaration - PPA-Europe - Double skin steel faced sandwich panels with a core made of polyurethane
HWD = Hazardous waste disposed; NHWD = Non-hazardous waste disposed; RWD = Radioactive waste disposed; CRU = Components for re-use;
MFR = Materials for recycling; MER = Materials for energy recovery; EEE = Exported electrical energy; EET = Exported thermal energy
RESULTS OF THE LCA – additional impact categories according to EN 15804+A2-optional:
1 m² PU sandwich panel 100 mm (12.6 kg/m²)
Parameter Unit A1-A3 A4 A5 C1 C2 C3 C4 D
Disease
PM 1.93E-06 8.45E-10 2.25E-10 9.51E-08 4.23E-10 1.46E-08 0 -4.25E-07
incidence
IR kBq U235 eq 7.64E-01 3.43E-04 1.48E-04 3.1E-03 1.72E-04 1.53E-02 0 -6.44E-01
ETP-fw CTUe 2.47E+02 8.71E-01 1.44E-02 7.87E+00 4.35E-01 7.95E-01 0 -3.07E+01
HTP-c CTUh 2.78E-08 1.78E-11 1.63E-12 1.61E-10 8.91E-12 6.13E-11 0 -2.27E-08
HTP-nc CTUh 4.55E-07 9.49E-10 2.23E-10 1.06E-08 4.74E-10 2.08E-09 0 -6.15E-08
SQP SQP 6.46E+01 5.12E-01 1.31E-02 4.63E+00 2.56E-01 5.15E-01 0 -1.32E+00
PM = Potential incidence of disease due to PM emissions; IR = Potential Human exposure efficiency relative to U235; ETP-fw = Potential comparative
Toxic Unit for ecosystems; HTP-c = Potential comparative Toxic Unit for humans (cancerogenic); HTP-nc = Potential comparative Toxic Unit for humans
(not cancerogenic); SQP = Potential soil quality index
Disclaimer 1 – concerning Potential Human exposure efficiency relative to U235 (IRP) - This impact category deals mainly with the
eventual impact of low-dose ionizing radiation on human health of the nuclear fuel cycle. It does not consider effects due to possible
nuclear accidents, occupational exposure or radioactive waste disposal in underground facilities. Potential ionizing radiation from the
soil, radon and from some construction materials is also not measured by this indicator.
Disclaimer 2 – concerning (ADP-minerals&metals, ADP-fossil, WDP, ETP-fwm HTP-c, HTP-nc, SQP) - The results of this
environmental impact indicator shall be used with care as the uncertainties on these results are high as there is limited experience with
the indicator.
References
EN 10169 Double skin metal faced sandwich panels, Institut Bauen und
Continuously organic coated (coil coated) steel flat products - Umwelt e.V., www.bau-umwelt.com, v8., October 2023
Technical delivery conditions
REACH
EN 10346 Regulation (EC) No 1907/2006 of the European Parliament and
Continuously hot-dip coated steel flat products for cold of the Council of 18 December 2006 concerning the
forming - Technical delivery conditions Registration, Evaluation, Authorisation and Restriction of
Chemicals
EN 13165
Thermal insulation products for buildings - Factory made rigid
polyurethane foam (PU) products - Specification
EN ISO 14044
Environmental management - Life cycle assessment -
Requirements and guidelines
EN 14509
Self-supporting double skin metal faced insulating panels -
Factory made products - Specifications
EN 15804+A2
EN 15804+A2:2019-04: Sustainability of construction works -
Environmental Product Declarations - Core rules for the product
category of construction products
CPR
REGULATION (EU) No 305/2011 OF THE EUROPEAN
PARLIAMENT AND OF THE COUNCIL of 9 March 2011 laying
down harmonised conditions for the marketing of construction
products and repealing Council Directive 89/106/EEC
LCA FE Software and Database
LCA FE software-system and CUP 2023.1 databases,
University of Stuttgart and Sphera Solutions GmbH, Leinfelden-
Echterdingen, 2023 (https://sphera.com/product-sustainability-
gabi-data-search/)
PCR - Part A
Calculation rules for the Life Cycle Assessment and
Requirements on the Background Report, v1.3, Institut Bauen
und Umwelt e.V., www.bau-umwelt.com, August 2021
PCR - Part B
6 Environmental Product Declaration - PPA-Europe - Double skin steel faced sandwich panels with a core made of polyurethane
7 Environmental Product Declaration - PPA-Europe - Double skin steel faced sandwich panels with a core made of polyurethane
Publisher
Institut Bauen und Umwelt e.V. +49 (0)30 3087748- 0
Hegelplatz 1 info@ibu-epd.com
10117 Berlin www.ibu-epd.com
Germany
Programme holder
Institut Bauen und Umwelt e.V. +49 (0)30 3087748- 0
Hegelplatz 1 info@ibu-epd.com
10117 Berlin www.ibu-epd.com
Germany
Author of the Life Cycle Assessment
Sphera Solutions GmbH +49 (0)711 341817-0
Hauptstraße 111- 113 info@sphera.com
70771 Leinfelden-Echterdingen www.sphera.com
Germany
Owner of the Declaration
European Association for Panels and Profiles e. V. +49 2151 93630-0
(PPA-Europe) info@ppa-europe.eu
Europark Fichtenhain A 13a www.ppa-europe.eu
47807 Krefeld
Germany
8 Environmental Product Declaration - PPA-Europe - Double skin steel faced sandwich panels with a core made of polyurethane
