ENVIRONMENTAL PRODUCT DECLARATION
as per ISO 14025 and EN 15804+A2
Owner of the Declaration ARGE – The European Federation of Locks and Building Hardware Manufacturers
Publisher Institut Bauen und Umwelt e.V. (IBU)
Programme holder Institut Bauen und Umwelt e.V. (IBU)
Declaration number EPD-ARG-20230545-IBG1-EN
Issue date 02.04.2024
Valid to 01.04.2029
Lock cylinders
ARGE – The European Federation of Locks
and Building Hardware Manufacturers
This EPD is valid only for products supplied by an ARGE EPD licence holder.
www.ibu-epd.com | https://epd-online.com
1. General Information
ARGE – The European Federation of Locks Lock cylinders
and Building Hardware Manufacturers
Programme holder Owner of the declaration
IBU – Institut Bauen und Umwelt e.V. ARGE – The European Federation of Locks and Building Hardware
Hegelplatz 1 Manufacturers
10117 Berlin Offerstraße 12
Germany 42551 Velbert
Germany
Declaration number Declared product / declared unit
EPD-ARG-20230545-IBG1-EN 1 kg of lock cylinder
This declaration is based on the product category rules: Scope:
Building Hardware products, 01.08.2021 This ARGE EPD covers cylinders which are used to operate locks by
(PCR checked and approved by the SVR) means of a key. The reference product used to calculate the impact this
product group has on the environment is a lock cylinder composed
primarily of brass, Zamak and steel, and has been selected for the LCA
Issue date (Life Cycle Assessment) because it is the product with the highest impact
for 1 kg of product. A validity scope analysis has also been carried out to
02.04.2024
determine the limiting factors for lock cylinders covered by this EPD. In a
preliminary study (simplified LCA), it has been confirmed that this EPD
represents the worst-case condition and it can therefore be used to cover
Valid to
all lock cylinders manufactured in Europe by ARGE member companies.
01.04.2029 The owner of the declaration shall be liable for the underlying information
and evidence; the IBU shall not be liable with respect to manufacturer
information, life cycle assessment data and evidences.
The EPD was created according to the specifications of EN 15804+A2. In
the following, the standard will be simplified as EN 15804.
Verification
The standard EN 15804 serves as the core PCR
Independent verification of the declaration and data according to ISO
14025:2011
Dipl.-Ing. Hans Peters internally X externally
(Chairman of Institut Bauen und Umwelt e.V.)
Florian Pronold Dr. Matthew Fishwick,
(Managing Director Institut Bauen und Umwelt e.V.) (Independent verifier)
1 Environmental Product Declaration - ARGE – The European Federation of Locks and Building Hardware Manufacturers - Lock cylinders
2. Product
2.1 Product description/Product definition Steel is produced by combining iron with carbon as well as
This EPD covers cylinders used to operate, by means of a key, other elements depending on the desired characteristics.
the bolt throwing mechanism in a lock. It covers lock cylinders Components made of steel are formed by stamping or other
with varying material compositions and security grades. types of mechanical processing.
For the application and use the respective national provisions
at the place of use apply. Sintered iron is produced by a process in which powdered
metal is pressed into a specific shape and then heated to bond
2.2 Application
the metal particles in the designed shape of the component.
These products are designed to be mounted in lock assemblies
consisting of various materials intended for use on interior or Nickel is a hard and ductile transition metal. Components can
exterior doors. be nickel-coated for decorative reasons and for providing
corrosion and wear resistance.
2.3 Technical Data
Products should comply with a suitable technical specification.
Nickel silver is an alloy of copper, nickel, and zinc.
EN 1303:2015, Building Hardware Cylinders for locks –
Components made of nickel silver are formed by stamping or
Requirements and test methods is an example of such a
other types of mechanical processing.
specification and most products will comply with it. The relevant
grading structure is shown in the following table:
Bronze is an alloy consisting primarily of copper, commonly
Name Value Unit
with tin and often with the addition of other metals and
Category of use 1 Grade sometimes non-metals. Components can be bronze-coated for
Durability 4 - 6 Grade decorative reasons and for providing sliding and dry running
Door mass 0 Grade properties.
Suitability for use in fire resisting and/or smoke
0, A, B Grade Stainless steel is produced by combining iron with chromium
control doors
as well as other elements depending on the desired
Safety 0 Grade
characteristics. Components made of steel are formed by
Corrosion resistance and temperature 0, A, B Grade stamping or other types of mechanical processing.
Key related security 1 - 6 Grade
0, A, B, Nylon 6 is a polymer, in particular polyamide. It is formed by
Attack resistance Grade
D the ring-opening polymerisation of caprolactam. Components
made of Nylon 6 are formed by injection moulding or other
Performance data of the product with respect to its
thermal forming processes.
characteristics in accordance with the relevant technical
provision (no CE-marking).
1) This product/article/at least one partial article contains
substances listed in the ECHA candidate list (date: 14.06.2023)
2.4 Delivery status
exceeding 0.1 percentage by mass: Certain components may
The products are sold by unit. Deliveries of individual items are
contain small amounts of lead (CAS no. 7439-92-1) as an
possible but are an exception. Standard deliveries comprise a
alloying element.
larger quantity of lock cylinders, as they are marketed as "B2B"
products and not to end-users.
2) This product/article/at least one partial article contains other
2.5 Base materials/Ancillary materials cancerogenic, mutagenic, reprotoxic (CMR) substances in
categories 1A or 1B which are not on the ECHA candidate list,
Composition of products analysed for this EPD:
exceeding 0.1 percentage by mass: no.
The values are given for the product analysed for this EPD.
3) Biocide products were added to this construction product or it
Ranges of values for other products covered by the validity
has been treated with biocide products (this then concerns a
scope analysis are shown in brackets.
treated product as defined by the (EU) Ordinance on Biocide
Name Value Unit
Products No. 528/2012): no.
Brass (24.88% – 92.61%) 67.62 %
2.6 Manufacture
Zamak (0.00% – 39.98%) 19.71 %
The manufacture of a lock cylinder usually follows a 3-step
Steel (4.15% – 41.48%) 10.34 %
process:
Sinter iron (0.00% – 2.81%) 2.25 %
1. Manufacture of the components: this step may include
Nickel (0.00% – 0.75%) 0 %
surface treatment in the factory or by external
Nickel silver (0.00% – 11.19%) 0 %
contractors.
Bronze (0.00% – 0.75%) 0 % 2. Pre-assembly of modules (in the factory).
Stainless steel (0.00% – 11.44%) 0 % 3. Final assembly (in the factory).
Nylon 6 (0.00% – 5.15%) 0 %
2.7 Environment and health during manufacturing
Brass is an alloy of zinc and copper. Components made of Regular measurements of air quality and noise levels are
brass are made by extrusion, forging, die-casting or other types carried out by the manufacturers, the ARGE member
of mechanical processing. companies. The results shall be within the mandatory safety
levels. In areas where employees are exposed to chemical
Zamak is an alloy with a base metal of zinc and alloying products, the required protective clothing and technical
elements of aluminium, magnesium, and copper. Components protective devices shall be provided. Regular health checks are
made of Zamak are die-cast. mandatory for employees in production facilities.
2 Environmental Product Declaration - ARGE – The European Federation of Locks and Building Hardware Manufacturers - Lock cylinders
done in line with instructions provided by the manufacturer.
2.8 Product processing/Installation
The installation of the product may vary depending on the type 2.13 Extraordinary effects
of lock assembly and the specific situation, but the products Fire
shall not require energy consumption for installation. The product is suitable for use in a fire resisting and/or smoke
control door set according to the classes specified in EN 1303,
2.9 Packaging unless it is classified in class/grade 0.
Normally, each individual product is packed in paper or
cardboard. These individual products are then packed in a Water
cardboard box and stacked on wooden pallets for transport to The declared product is intended to be used in buildings under
the customer. normal conditions (indoor or outdoor). It shall not emit
hazardous substances in the event of flooding.
Waste from product packaging is collected separately for waste
disposal (including recycling). Mechanical destruction
Mechanical destruction of the declared product shall not
2.10 Condition of use
materially alter its composition, or have any adverse effect on
Once installed, the products shall require no servicing during the environment.
their expected service lives. There shall be no consumption of
water or energy linked to their use, and they shall not cause 2.14 Re-use phase
any emissions. Removal of the cylinder (for recycling or re-use) shall have no
adverse effect on the environment.
2.11 Environment and health during use
No environmental damage or health risks are to be expected 2.15 Disposal
during normal conditions of use. Lock cylinders should be recycled wherever possible, providing
that there is no adverse effect on the environment. The waste
2.12 Reference service life
code in accordance with the European Waste Code is 17 04 07.
The reference service life is 30 years under normal working
conditions. This corresponds to passing a mechanical 2.16 Further information
endurance test of 100.000 cycles as specified in the EN 1303. Details of all types and variants can be found on the
The reference service life is dependent on the actual frequency manufacturers' websites. The respective website addresses are
of use and environmental conditions. It is required that available at https://arge.org.
installation, as well as maintenance of the product, must be
3. LCA: Calculation rules
The End-of-Life (EoL) stages are also considered. The
3.1 Declared Unit
transportation to the EoL disposal site is taken into account in
The declared unit for all products covered by ARGE EPD is 1 module C2. Module C4 covers the disposal of the locks.
kg (of product). Since individual products will rarely weigh Module C3 covers the recycling of the individual elements
exactly 1 kg it is necessary to establish the exact weight of the according to European averages, with the remaining waste
product and then use this as a correction factor to determine divided between incineration and landfill. Such a mixed
the true values for 1 kg of product in the tables (Section 5). scenario is declared due to the complex material mix of the
Declared unit product and the dependency of the EoL-route on the EoL-route
of the product the lock cylinder has been integrated into.
Name Value Unit
In practice, the end of life has been modelled as follows:
Declared unit 1 kg
• when a material is sent for recycling, generic transport
Mass of declared product 0.294 kg
and electric consumption of a shredder is taken into
Raw density 1 kg/m3 account (corresponding to the process 'Grinding,
metals'). Only then, is the material considered to have
attained the 'end-of-waste' state.
3.2 System boundary • each type of waste is modelled as a transport to the
Type of the EPD: "cradle to gate with options, with modules C1 treatment site with a distance of 30 km. Parts sent for
– C4, and module D (A1-A3, C1-C3, D and additional recycling include electricity consumption (grinding) and
modules)" a flow ('Materials for recycling, unspecified').
3.3 Estimates and assumptions
The analysis of the product life cycle includes the production
and transport of the raw materials, the manufacture of the The LCA data of the declared lock cylinder have been
product and the packaging materials which are declared in calculated from the production data of in total 4 ARGE member
modules A1-A3. companies, representing 8 different products. These companies
Losses during production are considered as waste and are sent had been chosen by ARGE as being representative by means
for recycling. No recycling processes are taken into account of their production processes and their market shares. The
except for transport and electricity consumption for grinding the product chosen as representative for this calculation follows the
metals. When recycled metals are used as raw material only "worst-case" principle as explained in section 6. LCA
their transformation process is taken into account and not the interpretation.
extraction of the raw material.
3.4 Cut-off criteria
A4 module represents the transport of the finished lock cylinder
The cut-off criteria considered are 1% of renewable and non-
to the installation site.
renewable primary energy usage and 1% of the total mass of
There is no waste associated with the installation of the
that unit process. The total neglected input flows per module
product. The A5 module therefore represents only the disposal
shall be a maximum of 5% of energy usage and mass.
of the product packaging.
3 Environmental Product Declaration - ARGE – The European Federation of Locks and Building Hardware Manufacturers - Lock cylinders
Technology: Material shaping technologies are based on
For this study, all input and output flows have been considered European technology in the case of the use of generic data.
at 100%, including raw materials as per the product
composition provided by the manufacturer and packaging of A total of 8 typical products (based on sales figures) have been
raw materials as well as the final product. Energy and water evaluated, and the worst-case results are used in the tables.
consumptions have also been considered at 100% according to
the data provided. 3.7 Period under review
The data of the LCA is based on the annual production data of
With the approach chosen, no significant environmental an ARGE member from 2013, considered representative for the
impacts are known to have been cut off. year 2022.
3.5 Background data 3.8 Geographic Representativeness
For the life cycle modelling of the considered product, all Land or region, in which the declared product system is
relevant background datasets are taken from ecoinvent v3.8 manufactured, used or handled at the end of the product´s
(system model: cut-off by classification). lifespan: Europe
3.6 Data quality
3.9 Allocation
The objective of this evaluation is to evaluate the environmental
impacts generated by the products throughout their entire life The products are produced in numerous production sites. All
cycles. To this end, ISO 14040, ISO 14044 and EN 15804 have data were provided by the manufacturers of the products per
been met regarding the quality of data on the following different unit and then divided by the mass of the product to give a value
criteria: per kg of product produced.
Time: The life cycle inventory data used come from: The assumptions relating to the EoL of the product are
described in the section System Boundaries.
• Data collected specifically for this study on the ARGE
member companies' manufacturing sites. Datasets are
Metal losses during production (stage A3) are considered as
based on 1-year averaged data (time period: January
waste.
2013 to December 2013 considered representative for
2022). 3.10 Comparability
• In the absence of collected data, generic data from the
Basically, a comparison or an evaluation of EPD data is only
ecoinvent v3.8 database have been used. This is
possible if all the data sets to be compared were created
updated regularly and is representative of current
according to EN 15804 and the building context, respectively
processes (the entire database having been updated in
the product-specific characteristics of performance, are taken
2021).
into account.
Geography: Data come from production sites of the ARGE
member companies. Generic data come from the ecoinvent
ecoinvent v3.8 (system model: cut-off by classification) has
database, representative for European production processes.
been used as the background database.
4. LCA: Scenarios and additional technical information
been taken into account.
Characteristic product properties of biogenic carbon
End of life packaging is a mix between recycling, landfill and
Information on the biogenic carbon content at factory gate incineration according to French ADEME statistics.
Note: 1 kg of biogenic carbon is equivalent to 44/12 kg of CO .
2
No re-use of packaging is considered in this study.
Name Value Unit
kg
Biogenic carbon content in product 0
C
Reference service life
Biogenic carbon content in accompanying kg
0.0595 Name Value Unit
packaging C
Reference service life 30 a
Test cycles over RSL (EN 1303) 100'000 cycles
The following information is the basis of the declared modules
within the LCA in this EPD. End of life (C1-C4)
Transport to the building site (A4) Name Value Unit
Name Value Unit Collected separately waste type 1 kg
Litres of fuel 25.8 l/100km Recycling 0.458 kg
Transport distance 3500 km Energy recovery 0.249 kg
Capacity utilisation (including empty runs) 36 % Landfilling 0.293 kg
It is assumed that a 16–32-ton truck is used to transport the
Installation into the building (A5)
product:
Name Value Unit
- Transport to shredding facility for metal recovery: 150 km
Material loss 0.137 kg - Transport to municipal waste incineration plant: 50 km
The scope of this study does not cover the installation of the - Transport to landfill: 30 km
product, which varies depending on the type of door and the
specific situation. The disposal of the product packaging has Reuse, recovery and/or recycling potentials (D), relevant
4 Environmental Product Declaration - ARGE – The European Federation of Locks and Building Hardware Manufacturers - Lock cylinders
scenario information recycling (MFR);
- net amounts of a metal leaving the product system are
Module D contains the benefits and loads beyond the system quantified as the material for recycling leaving modules A1-C4
boundary related to the recycling of metals, which result from minus the input of secondary scrap (secondary material, SM) to
the treatment of recycled materials from the point of end-of- the product system;
waste status to the point of substitution (as costs) and the - in the case of brass and zinc alloys, which are composed of
substitution of primary resources (as benefits). two different constituting metals, no difference shall be made
between the input of secondary constituting metals (Cu and Zn;
According to EN 16710, clause 6.4.3.3: 'In module D Cu and Sn) and its alloys (CuZn; CuSn).
substitution effects are calculated only for the resulting net
output flow. Negative net output flows have not been considered in the
quantification of module D.
For building hardware, the following rules apply for the
quantification of net output flows: It also includes the benefits and loads related to 'exported
- all production scrap and cuttings leave modules A1-B3 as energy electricity' and 'exported energy heat' resulting from the
sorted scrap without allocated burdens from primary production; energy recovery from plastic wastes in a municipal waste
the corresponding amounts are declared as material for incineration plant as modelled in Modules A3, A5 and C4.
5 Environmental Product Declaration - ARGE – The European Federation of Locks and Building Hardware Manufacturers - Lock cylinders
5. LCA: Results
In Table 1 "Description of the system boundary", the declared modules are indicated with an "X"; all modules that are not declared
within the EPD but where additional data are available are indicated with "MND". Those data can also be used for building assessment
scenarios. The values are declared with three valid digits in exponential form.
The set of characterisation factors EF3.0 has been used for the life cycle assessment.
DESCRIPTION OF THE SYSTEM BOUNDARY (X = INCLUDED IN LCA; MND = MODULE OR INDICATOR NOT DECLARED; MNR
= MODULE NOT RELEVANT)
Benefits and
Construction loads beyond
Product stage Use stage End of life stage
process stage the system
boundaries
la ire wta am R y lp p u s tro p s n a rT g n iru tc a fu n a M tro p s nm ae o rh r
T
f te tis e h t o t e ta g y lb m e s s A e s U e c n a n e tn ia M ria p e R tn e m e c a lp e R tn e m h s ib ru fe R la n o ity ag rr ee pn Oe e s u la n o ita r re et pa Ow e s u n o itc u rts n eo Dc -n o itilo m e d tro p s n a rT g n is s ee tsc ao Wrp la s o p s iD e s u e R- y re v o c e R- g n ilc y c e R- la itn e to p
A1 A2 A3 A4 A5 B1 B2 B3 B4 B5 B6 B7 C1 C2 C3 C4 D
X X X X X MND MND MNR MNR MNR MND MND X X X X X
RESULTS OF THE LCA - ENVIRONMENTAL IMPACT according to EN 15804+A2: 1 kg of lock cylinder
Parameter Unit A1-A3 A4 A5 C1 C2 C3 C4 D
GWP-total kg CO2 eq 1.09E+01 6.52E-01 2.22E-01 0 1.5E-02 3.12E-03 4.64E-03 -5.25E+00
GWP-fossil kg CO2 eq 1.11E+01 6.51E-01 3.36E-03 0 1.5E-02 3.11E-03 4.63E-03 -5.24E+00
GWP-biogenic kg CO2 eq -2.18E-01 0 2.18E-01 0 0 0 0 0
GWP-luluc kg CO2 eq 2.34E-02 2.61E-04 1.23E-06 0 5.98E-06 7.76E-06 3.8E-06 -1.19E-02
ODP kg CFC11 eq 7.53E-07 1.51E-07 6.88E-10 0 3.47E-09 1.58E-10 1.33E-09 -2.84E-07
AP mol H+ eq 5.91E-01 1.85E-03 1.48E-05 0 4.25E-05 1.6E-05 3.35E-05 -3.37E-01
EP-freshwater kg P eq 2.7E-03 4.65E-06 2.85E-08 0 1.07E-07 3.49E-07 6.67E-08 -1.51E-03
EP-marine kg N eq 3.25E-02 3.68E-04 4.93E-06 0 8.44E-06 2.05E-06 1.11E-05 -1.69E-02
EP-terrestrial mol N eq 4.44E-01 4.1E-03 5.32E-05 0 9.41E-05 2.37E-05 1.23E-04 -2.41E-01
kg NMVOC
POCP 1.22E-01 1.58E-03 1.55E-05 0 3.62E-05 6.49E-06 3.75E-05 -6.67E-02
eq
ADPE kg Sb eq 1.46E-02 2.31E-06 1.12E-08 0 5.3E-08 7.54E-09 1.46E-08 -8.45E-03
ADPF MJ 1.39E+02 9.88E+00 4.67E-02 0 2.27E-01 6.59E-02 9.95E-02 -6.39E+01
m3 world eq
WDP 1.09E+01 3.01E-02 2.34E-04 0 6.9E-04 7.36E-04 -5.9E-04 -5.94E+00
deprived
GWP = Global warming potential; ODP = Depletion potential of the stratospheric ozone layer; AP = Acidification potential of land and water; EP =
Eutrophication potential; POCP = Formation potential of tropospheric ozone photochemical oxidants; ADPE = Abiotic depletion potential for non-fossil
resources; ADPF = Abiotic depletion potential for fossil resources; WDP = Water (user) deprivation potential)
RESULTS OF THE LCA - INDICATORS TO DESCRIBE RESOURCE USE according to EN 15804+A2: 1 kg of lock cylinder
Parameter Unit A1-A3 A4 A5 C1 C2 C3 C4 D
PERE MJ 3E+01 1.39E-01 -7.08E-01 0 3.19E-03 1.25E-02 1.41E-03 -1.56E+01
PERM MJ 1.79E+00 0 -2.19E-01 0 0 0 0 0
PERT MJ 3.18E+01 1.39E-01 -9.28E-01 0 3.19E-03 1.25E-02 1.41E-03 -1.56E+01
PENRE MJ 1.4E+02 9.88E+00 4.67E-02 0 2.27E-01 6.65E-02 9.95E-02 -6.41E+01
PENRM MJ 0 0 0 0 0 0 0 0
PENRT MJ 1.4E+02 9.88E+00 4.67E-02 0 2.27E-01 6.65E-02 9.95E-02 -6.41E+01
SM kg 2.79E-01 0 0 0 0 0 0 0
RSF MJ 0 0 0 0 0 0 0 0
NRSF MJ 0 0 0 0 0 0 0 0
FW m3 2.07E-01 1.05E-03 3.85E-05 0 2.41E-05 4.25E-05 2.16E-04 -1.07E-01
PERE = Use of renewable primary energy excluding renewable primary energy resources used as raw materials; PERM = Use of renewable primary
energy resources used as raw materials; PERT = Total use of renewable primary energy resources; PENRE = Use of non-renewable primary energy
excluding non-renewable primary energy resources used as raw materials; PENRM = Use of non-renewable primary energy resources used as raw
materials; PENRT = Total use of non-renewable primary energy resources; SM = Use of secondary material; RSF = Use of renewable secondary fuels;
NRSF = Use of non-renewable secondary fuels; FW = Use of net fresh water
RESULTS OF THE LCA – WASTE CATEGORIES AND OUTPUT FLOWS according to EN 15804+A2:
1 kg of lock cylinder
Parameter Unit A1-A3 A4 A5 C1 C2 C3 C4 D
HWD kg 4.07E-03 2.58E-05 1.97E-07 0 5.92E-07 2.34E-08 1.88E-07 -2.34E-03
NHWD kg 5.44E+00 5.2E-01 2.91E-03 0 1.19E-02 2.48E-04 4.15E-01 -2.4E+00
RWD kg 9.68E-04 1.43E-04 6.28E-07 0 3.28E-06 8.86E-07 1.28E-06 -3.76E-04
CRU kg 0 0 0 0 0 0 0 0
MFR kg 7.94E-01 0 9.86E-02 0 0 4.66E-01 0 0
MER kg 0 0 0 0 0 0 0 0
6 Environmental Product Declaration - ARGE – The European Federation of Locks and Building Hardware Manufacturers - Lock cylinders
EEE MJ 0 0 2.47E-02 0 0 0 0 0
EET MJ 0 0 1.64E-01 0 0 0 0 0
HWD = Hazardous waste disposed; NHWD = Non-hazardous waste disposed; RWD = Radioactive waste disposed; CRU = Components for re-use;
MFR = Materials for recycling; MER = Materials for energy recovery; EEE = Exported electrical energy; EET = Exported thermal energy
RESULTS OF THE LCA – additional impact categories according to EN 15804+A2-optional:
1 kg of lock cylinder
Parameter Unit A1-A3 A4 A5 C1 C2 C3 C4 D
Disease
PM 1.49E-06 5.23E-08 2.96E-10 0 1.2E-09 4.28E-11 1.01E-09 -7.86E-07
incidence
IR kBq U235 eq 6.46E-01 4.29E-02 1.91E-04 0 9.84E-04 6E-04 3.83E-04 -2.9E-01
ETP-fw CTUe 4.87E+03 7.75E+00 4.18E-02 0 1.78E-01 3.32E-02 5.09E-01 -2.79E+03
HTP-c CTUh 1.16E-07 2.49E-10 2.71E-12 0 5.72E-12 8.86E-13 7.29E-12 -6.48E-08
HTP-nc CTUh 7.92E-06 7.83E-09 1.11E-10 0 1.8E-10 2.88E-11 8.44E-11 -4.55E-06
SQP SQP 2.35E+02 6.88E+00 3.07E-02 0 1.58E-01 1.01E-02 1.7E-01 -1.12E+02
PM = Potential incidence of disease due to PM emissions; IR = Potential Human exposure efficiency relative to U235; ETP-fw = Potential comparative
Toxic Unit for ecosystems; HTP-c = Potential comparative Toxic Unit for humans (cancerogenic); HTP-nc = Potential comparative Toxic Unit for humans
(not cancerogenic); SQP = Potential soil quality index
Disclaimer 1 –
for the indicator 'Potential Human exposure efficiency relative to U235'. This impact category deals mainly with the eventual impact of
low-dose ionizing radiation on human health of the nuclear fuel cycle. It does not consider effects due to possible nuclear accidents,
occupational exposure or radioactive waste disposal in underground facilities. Potential ionizing radiation from the soil, radon and from
some construction materials is also not measured by this indicator.
Disclaimer 2 –
for the indicators 'abiotic depletion potential for non-fossil resources', 'abiotic depletion potential for fossil resources', 'water (user)
deprivation potential, deprivation-weighted water consumption', 'potential comparative toxic unit for ecosystems', 'potential comparative
toxic unit for humans – cancerogenic', 'Potential comparative toxic unit for humans - not cancerogenic', 'potential soil quality index'. The
results of this environmental impact indicator shall be used with care as the uncertainties on these results are high as there is limited
experience with the indicator.
6. LCA: Interpretation
Figure 1 illustrates the relative contributions of the different
modules along the life cycle of the declared products.
significant.
Figure 1: Environmental impacts of lock cyclinders along
its life cycle Benefits and burdens beyond the system boundary (module D)
are in the order of 25 % to 35 % of the impacts over the product
The largest part of environmental impacts is caused during life cycle (modules A1-A3) and relate basically to the recycling
production (modules A1-A3); comparably small impacts are of metals.
caused during the transport of the product to the construction
site (via the manufacturer of the product, which the lock cylinder A total of 8 typical products (based on sales figures) have been
has been integrated into). evaluated and the worst-case results are used in section 5 of
this EPD. In chapter 2.5, the tabulated range of relative weight
All the other modules related to the product life cycle are not per material ensures that the variability of results stays within
7 Environmental Product Declaration - ARGE – The European Federation of Locks and Building Hardware Manufacturers - Lock cylinders
+/- 40% of the declared values (assessed for the indicators GWP, PENRT, and non-hazardous waste).
7. Requisite evidence
No testing results are required by the PCR part B.
8. References
Product category rules of IBU DIN EN 1303:2015, Building hardware - Cylinders for locks -
Requirements and test methods.
IBU (2021)
IBU (2021): General Instructions for the EPD Programme of the EN 13501-1
Institut Bauen und Umwelt e.V. (General Instructions for the EN 13501-1:2018, Fire classification of construction products
IBU EPD Programme). Version 2.0, Institut Bauen und Umwelt, and building elements - Part 1: Classification using data from
Berlin. reaction to fire tests.
IBU (2021) ISO 15686
IBU (2021) PCR Part A: Calculation rules for the life cycle ISO 15686:1, -2, -7 and -8. Service life planning (various parts).
assessment and requirements on the project report according
to EN 15804+A2. Version 1.3., Institut Bauen und Umwelt, ECHA candidate list
Berlin. Candidate List of substances of very high concern for
Authorisation, published in accordance with Article 59(10) of the
IBU (2023) REACH Regulation. European Chemicals Agency, Brussels.
IBU (2023): PCR Part B: Requirements on the EPD for building
hardware products, Institut Bauen und Umwelt, Berlin. Ordinance on Biocide Products No. 528/2012
REGULATION (EU) No 528/2012 OF THE EUROPEAN
Standards and legal documents PARLIAMENT AND OF THE COUNCIL of 22 May 2012
concerning the making available on the market and use of
EN 15804 biocidal products.
EN 15804:2012+A2:2019+AC:2021, Sustainability of
construction works - Environmental product declarations - Core European List of Waste
rules for the product category of construction products. Commission Decision of 3 May 2000 replacing Decision
94/3/EC establishing a list of wastes pursuant to Article 1(a) of
EN 17610 Council Directive 75/442/EEC on waste and Council Decision
EN 17610:2022, Building hardware - Environmental product 94/904/EC establishing a list of hazardous waste pursuant to
declarations - Product category rules complementary to EN Article 1(4) of Council Directive 91/689/EEC on hazardous
15804 for building hardware. waste (notified under document number C(2000) 1147).
ISO 14025 Additional references
ISO 14025:2006-07, Environmental labels and declarations -
Type III Environmental declarations - Principles and BBSR 2017
procedures. BBSR (2017): Nutzungsdauer von Bauteilen in
Lebenszyklusanalysen nach Bewertungssystem Nachhaltiges
ISO 14044 Bauen (BNB). Version vom 24.10.2017, Bundesinstitut für Bau-,
EN ISO 14044:2006-07, Environmental management - Life Stadt- und Raumforschung, Berlin.
cycle assessment - Requirements and guidance (ISO
14044:2006). ecoinvent v3.8
http://www.ecoinvent.org
EN 1303
8 Environmental Product Declaration - ARGE – The European Federation of Locks and Building Hardware Manufacturers - Lock cylinders
Publisher
Institut Bauen und Umwelt e.V. +49 (0)30 3087748- 0
Hegelplatz 1 info@ibu-epd.com
10117 Berlin www.ibu-epd.com
Germany
Programme holder
Institut Bauen und Umwelt e.V. +49 (0)30 3087748- 0
Hegelplatz 1 info@ibu-epd.com
10117 Berlin www.ibu-epd.com
Germany
Author of the Life Cycle Assessment
Dr. Frank Werner - Umwelt & Entwicklung + 41 (0)44 241 39 06
Kammelenbergstrasse 30 frank@frankwerner.ch
9011 St. Gallen http://www.frankwerner.ch/
Switzerland
Owner of the Declaration
ARGE – The European Federation of Locks and +49 (0)2051 9506 15
Building Hardware Manufacturers mail@arge.org
Offerstraße 12 www.arge.org
42551 Velbert
Germany
9 Environmental Product Declaration - ARGE – The European Federation of Locks and Building Hardware Manufacturers - Lock cylinders
