ENVIRONMENTAL PRODUCT DECLARATION
as per ISO 14025 and EN 15804
Owner of the Declaration ArcelorMittal Europe – Flat Products
Programme holder Institut Bauen und Umwelt e.V. (IBU)
Publisher Institut Bauen und Umwelt e.V. (IBU)
Declaration number EPD-ARC-20200038-CBA1-EN
ECO EPD Ref. No. ECO-00001206
Issue date 10.07.2020
Valid to 09.07.2025
Heavy Steel Plates
ArcelorMittal Europe
www.ibu-epd.com | https://epd-online.com
Umwelt Produktdeklaration Name des Herstellers – Name des Produkts
General Information
ArcelorMittal Europe Heavy Steel Plates
Programme holder Owner of the declaration
IBU – Institut Bauen und Umwelt e.V. ArcelorMittal Europe – Flat Products
Panoramastr. 1 24-26 Boulevard d’Avranches
10178 Berlin L-1160 Luxembourg
Germany Luxembourg
Declaration number Declared product / declared unit
EPD-ARC-20200038-CBA1-EN The declaration applies to 1 metric ton of Heavy Plate.
This declaration is based on the product Scope:
category rules: The Life Cycle Assessment is based on data collected
Structural steels, 07.2014 from the ArcelorMittal plant in Aviles/Gijon in Spain
(PCR checked and approved by the SVR) producing Heavy Plates, representing 100 % of the
annual production from 2018.
Issue date
10.07.2020 The owner of the declaration shall be liable for the
underlying information and evidence; the IBU shall not
be liable with respect to manufacturer information, life
Valid to
cycle assessment data and evidences.
09.07.2025
Verification
The standard EN 15804 serves as the core PCR
Independent verification of the declaration and data
according to ISO 14025:2010
Dipl. Ing. Hans Peters internally x externally
(chairman of Institut Bauen und Umwelt e.V.)
Dr. Alexander Röder Mr Carl-Otto Neven
(Managing Director Institut Bauen und Umwelt e.V.)) (Independent verifier appointed by SVR)
Product
Product description/Product definition Application
This Environmental Product Declaration refers to Heavy plates for construction can be used in various
heavy plates, hot rolled products produced on construction applications, such as:
dedicated quarto plate mill. Steel grade range for  Buildings: structural and built-up welded
construction include low alloy structural steels, as- sections, trusses, box girders, for heavy
rolled, normalized and thermomechanically rolled,
industrial steel frames, high rise buildings,
including weathering steels.
long-span structures for transport terminals
and other infrastructure.
Mean thickness value is at 20 mm but the declaration
covers the whole range from 5 mm up to 100 mm.  Road and railway bridges: steel & composite
Width range is from 1400 mm up to 3300 mm. structures made of welded built-up sections or
box girders or trusses, arch and bow-string
Weathering steels offer improved resistance to
bridges, pedestrian and bicycles bridges,
corrosion thanks to the addition of copper during
cable-stayed and suspension deck & pylons
manufacture. Additional alloying elements can be
bridges.
added to increase the steel’s tensile strength or make
forming processes easier.  Art sculpture.
For the placing of the product on the market in
Heavy Plates can be processed by conventional
the European Union/European Free Trade Association
processing operations used for steelwork fabrication:
(EU/EFTA) (with the exception of Switzerland)
oxy-cutting, bending, drilling, welding etc.
Regulation (EU) No. 305/2011 (CPR) applies. The
product has a declaration of performance taking into
When weathering steel is exposed to the ambient
consideration EN 10025-1:2004 - Hot rolled products
atmosphere it develops an initial layer of iron oxide in
of structural steels - Part 1: General technical delivery
the same way as carbon steel. The rate of oxidisation
conditions. For the application and use the respective
depends on how much oxygen, moisture, and
national provisions apply.
atmospheric contaminants can access the surface of
the metal. In the initial stages, a complex mix of iron
oxides covers the surface to create a layer of rust. As
2 Environmental Product Declaration ArcelorMittal – Heavy steel plates
the process progresses, the rust layer forms a barrier The metallurgical composition of weathering steels
against the corrosive agents and the rate of corrosion includes less than 0.2 % carbon. Alloying elements
slows. (mainly copper, chromium, nickel, phosphorus, silicon,
and manganese) typically comprise less than 5% of
Technical Data the steel. Due to their specific chemistry, the corrosion
ArcelorMittal offers a full range of grades in compliance rate of weathering steels is generally much lower than
with the EN 10025-1 and EN 10025 - part 2 to 5 to that of standard carbon steel. The possible chemical
meet different applications. compositions are defined in European standard.
Weathering steels can be classified into two
ArcelorMittal has also created different grades of categories: those with limited phosphorous content
weathering steels to meet different applications. Their (typically less than 0.035 %); and those with a higher
chemical composition and mechanical performance phosphorous content. Weathering steels with a
are specified in EN 10025-5. Yield strengths from 235 phosphorous content of between 0.06 and 0.15 % are
MPa up to 460 MPa are available. identified by the letter P at the end of the product
name.
ArcelorMittal Europe Flat products is producing heavy
plates in one mill located in Gijon in Spain. High levels of phosphorous improve the corrosion
resistance of weathering steels. Phosphorous is not
Constructional data used in heavy plate for structural uses as it can form
Name Value Unit iron phosphide (FeP3) during welding. This can
Density 7850 kg/m3 hamper weldability and cause the weld zone to
Modulus of elasticity 210000 N/mm2 become brittle. For this reason, phosphorous
Coefficient of thermal expansion 12 10-6K-1 weathering steels are usually only available in
Thermal conductivity 48 W/(mK) thicknesses lower than 12 mm.
1500 -
Melting point °C
1540 This product contains substances listed in the
Minimum yield strength 235 - 460 N/mm² candidate list (date: 26.2.2020) exceeding 0.1
percentage by mass: no.
Performance data of the product in accordance with
the declaration of performance with respect to its Reference service life
essential characteristics according to EN 10025-1 - Hot A reference service life for heavy steel plate is not
rolled products of structural steels - Part 1: General declared. Heavy steel plates are construction products
technical delivery conditions. For the application and with many different application purposes. The lifetime
use the respective national provisions apply. therefore will be limited by the application as well as
the service life of the work.
Base materials/Ancillary materials
The basic materials for the manufacture of Bridges using heavy plates are designed and
ArcelorMittal’s heavy steel plates are non-alloyed and calculated according to Eurocodes to ensure more
fine grain steel. Different steel grades and qualities are than 100 years of durability.
possible, these being recorded in the specific product
standards EN 10025-1 and EN 10025-2 or EN 10025-3 First structural steel projects using weathering steel
or EN 10025-4 or EN 10025-5. were completed 50 years ago in Europe and have
demonstrated a very low maintenance level and no
Steel is mainly iron and carbon, with small amounts of need for painting.
alloying elements. These elements modify the
chemical and physical properties of steel such as At the end of life, weathering steel products could be
strength, durability and corrosion resistance. High recovered, recycled and sent to the steel mill.
strength low alloyed (HSLA) carbon steel has a carbon
content lower than 0.2 %.
LCA: Calculation rules
Declared Unit Module A1-A3, Module C3 and module D were
This Environmental Product Declaration refers to considered.
Heavy Steel Plates including weathering steel, as
specified in Part B requirements on the EPD for Modules A1-A3 of the Heavy Steel Plates, including
Structural Steels. weathering steel range production include the
following:
Declared unit · The provision of resources, additives, and energy
Name Value Unit · Transport of resources and additives to the
Declared unit 1000 kg production site
Conversion factor to 1 kg 0.001 - · Production processes on-site including energy,
Density 7850 kg/m3 production of additives, disposal of production
residues, and consideration of related emissions
· Recycling of production/manufacturing scrap. Steel
scrap is assumed to reach the end-of-waste status
System boundary once it is shredded and sorted, thus becomes input to
Type of the EPD: cradle-to-gate - with options. the product system in the inventory.
3 Environmental Product Declaration ArcelorMittal – Heavy steel plates
Comparability
Module C3 takes into account the sorting and Basically, a comparison or an evaluation of EPD data
shredding of after-use steel that is recycled, as well as is only possible if all the data sets to be compared
the non-recovered scrap due to sorting efficiency were created according to EN 15804 and the building
which is landfilled. A conservative value of 2 % landfill context, respectively the product-specific
is considered. characteristics of performance, are taken into account.
Gabi version 9.2 was used with Gabi Database SP39
Module D refers to the End-of-Life of the heavy steel version 8.7 to calculate this EPD.
plates, including reuse and recycling.
LCA: Scenarios and additional technical information
Current practice for the average Heavy Steel Plates
consists of 98 % recycling and 2 % landfill according to
the European Commission Technical Steel Research.
End of life (C3)
Name Value Unit
Landfilling 2 %
Reuse, recovery and/or recycling potentials (D),
relevant scenario information
Name Value Unit
Recycling 98 %
4 Environmental Product Declaration ArcelorMittal – Heavy steel plates
LCA: Results
DESCRIPTION OF THE SYSTEM BOUNDARY (X = INCLUDED IN LCA; MND = MODULE NOT DECLARED;
MNR = MODULE NOT RELEVANT)
BENEFITS AND
CONSTRUCTI LOADS
PRODUCT STAGE ON PROCESS USE STAGE END OF LIFE STAGE BEYOND THE
STAGE SYSTEM
BOUNDARIES
5 Environmental Product Declaration ArcelorMittal – Heavy steel plates
lairetam
waR
ylppus tropsnarT
gnirutcafunaM
eht
morf
tropsnarT
etis
eht
ot
etag
ylbmessA esU
ecnanetniaM
riapeR
tnemecalpeR tnemhsibrufeR
ygrene
lanoitarepO esu
retaw
lanoitarepO esu
noitcurtsnoc-eD
noitilomed tropsnarT
gnissecorp
etsaW
lasopsiD -esueR -yrevoceR -gnilcyceR laitnetop
A1 A2 A3 A4 A5 B1 B2 B3 B4 B5 B6 B7 C1 C2 C3 C4 D
X X X MND MND MND MND MNR MNR MNR MND MND MND MND X MND X
RESULTS OF THE LCA - ENVIRONMENTAL IMPACT: 1 ton of heavy steel plate
Parameter Unit A1-A3 C3 D
Global warming potential [kg CO2-Eq.] 2.60E+3 1.99E+0 -1.80E+3
Depletion potential of the stratospheric ozone layer [kg CFC11-Eq.] 1.21E-12 4.48E-14 1.12E-11
Acidification potential of land and water [kg SO2-Eq.] 4.76E+0 6.28E-3 -4.21E+0
Eutrophication potential [kg (PO4)3--Eq.] 4.58E-1 7.23E-4 -3.59E-1
Formation potential of tropospheric ozone photochemical oxidants [kg ethene-Eq.] 8.93E-1 4.70E-4 -5.47E-1
Abiotic depletion potential for non-fossil resources [kg Sb-Eq.] 8.08E-5 4.99E-7 4.27E-5
Abiotic depletion potential for fossil resources [MJ] 2.35E+4 2.28E+1 -1.43E+4
RESULTS OF THE LCA - RESOURCE USE: 1 ton of heavy steel plate
Parameter Unit A1-A3 C3 D
Renewable primary energy as energy carrier [MJ] 6.21E+2 1.18E+1 1.49E+3
Renewable primary energy resources as material utilization [MJ] 0.00E+0 0.00E+0 0.00E+0
Total use of renewable primary energy resources [MJ] 6.21E+2 1.18E+1 1.49E+3
Non-renewable primary energy as energy carrier [MJ] 2.37E+4 3.42E+1 -1.35E+4
Non-renewable primary energy as material utilization [MJ] 0.00E+0 0.00E+0 0.00E+0
Total use of non-renewable primary energy resources [MJ] 2.37E+4 3.42E+1 -1.35E+4
Use of secondary material [kg] 4.22E+1 0.00E+0 0.00E+0
Use of renewable secondary fuels [MJ] 0.00E+0 0.00E+0 0.00E+0
Use of non-renewable secondary fuels [MJ] 0.00E+0 0.00E+0 0.00E+0
Use of net fresh water [m³] 5.23E+0 1.44E-2 -1.41E+0
RESULTS OF THE LCA – OUTPUT FLOWS AND WASTE CATEGORIES:
1 ton of heavy steel plate
Parameter Unit A1-A3 C3 D
Hazardous waste disposed [kg] 1.01E-5 2.05E-7 -8.98E-6
Non-hazardous waste disposed [kg] 7.58E+0 2.00E+1 -2.82E+1
Radioactive waste disposed [kg] 1.01E-1 4.54E-3 2.89E-1
Components for re-use [kg] 0.00E+0 0.00E+0 0.00E+0
Materials for recycling [kg] 0.00E+0 9.80E+2 0.00E+0
Materials for energy recovery [kg] 0.00E+0 0.00E+0 0.00E+0
Exported electrical energy [MJ] 0.00E+0 0.00E+0 0.00E+0
Exported thermal energy [MJ] 0.00E+0 0.00E+0 0.00E+0
References
EN 10025-1 to 5 structural steels with improved atmospheric corrosion
EN 10025-1:2004 - Hot rolled products of structural resistance
steels - Part 1: General technical delivery conditions
EN 10025-2:2019 - Hot rolled products of structural Institut Bauen und Umwelt
steels - Part 2: Technical delivery conditions for non- Institut Bauen und Umwelt e.V., Berlin (pub.):
alloy structural steels Generation of Environmental Product Declarations
EN 10025-3:2019 - Hot rolled products of structural (EPDs)
steels - Part 3: Technical delivery conditions for
normalized/normalized rolled weldable fine grain PCR Part B
structural steels PCR – Part B: Requirements of the EPD for Structural
EN 10025-4:2019 - Hot rolled products of structural steels,
steels - Part 4: Technical delivery conditions for Institut Bauen und Umwelt e.V., www.bauumwelt.com,
thermomechanical rolled weldable fine grain structural 2017
steels
EN 10025-5:2019 - Hot rolled products of structural ISO 14025
steels - Part 5: Technical delivery conditions for DIN EN ISO 14025:2011-10: Environmental labels and
declarations — Type III environmental declarations —
Principles and procedures GaBi ts Documentation
Documentation of the GaBi datasets for Life Cycle
EN 15804 Engineering. LBP, Universitity of Stuttgart and PE
EN 15804:2012-04+A1 2013: Sustainability of International, 2017.
construction works — Environmental Product http://documentation.gabi-software.com
Declarations — Core rules for the product category of
construction products REACH
Regulation (EC) No 1907/2006 of the European
European Commission Technical Steel Parliament and of the Council on the Registration,
Research Evaluation, Authorisation and Restriction
Sansom, M.and Meijer, J.:Life-cycle of Chemicals (REACH)
assessment (LCA) for steel construction, European https://echa.europa.eu/regulations/reach/legislation
Commission technical steel research, 2001-12
GaBi ts Software
GaBi ts. Software and Databases
LBP, University of Stuttgart
und PE International, 2017.
6 Environmental Product Declaration ArcelorMittal – Heavy steel plates
Publisher
Institut Bauen und Umwelt e.V. Tel +49 (0)30 3087748- 0
Panoramastr. 1 Fax +49 (0)30 3087748- 29
10178 Berlin Mail info@ibu-epd.com
Germany Web www.ibu-epd.com
Programme holder
Institut Bauen und Umwelt e.V. Tel +49 (0)30 - 3087748- 0
Panoramastr 1 Fax +49 (0)30 – 3087748 - 29
10178 Berlin Mail info@ibu-epd.com
Germany Web www.ibu-epd.com
Author of the Life Cycle
Assessment Tel +352 4792-1
ArcelorMittal Europe – Flat Products Fax -
Boulevard d’Avranches 24-26 Mail
1160 Luxembourg flateurope.technical.assistance
Luxembourg @arcelormittal.com
Web flateurope.arcelormittal.com/
Owner of the Declaration
ArcelorMittal Europe – Flat Products Tel +352 4792-1
Boulevard d’Avranches 24-26 Fax -
1160 Luxembourg Mail
Luxembourg flateurope.technical.assistance
@arcelormittal.com
Web flateurope.arcelormittal.com/
