Environmental product declaration
in accordance with ISO 14025 and EN 15804+A2
Self-levelling compounds StoCrete CS 730 and StoCrete CS 735
Owner of the declaration: Program operator:
Sto SE & Co. KGaA The Norwegian EPD Foundation
Product: Declaration number:
Self-levelling compounds StoCrete CS 730 and StoCrete
CS 735 NEPD-8924-8584
Declared unit: Registration number:
1 kg
NEPD-8924-8584
This declaration is based on Product Category Rules:
Issue date: 04.02.2025
CEN Standard EN 15804:2012+A2:2019 serves as core
The Norwegian EPD Foundation PCR Valid to: 04.02.2030
NPCR 009:2021 Part B for Technical - Chemical products
for building and construction industry EPD software:
LCAno EPD generator ID: 610209
1 / 12
General information
Product Owner of the declaration:
Self-levelling compounds StoCrete CS 730 and StoCrete CS 735 Sto SE & Co. KGaA
Contact person: Linus Kaltenbach
Phone: +49 7744571010
e-mail: l.kaltenbach@sto.com
Program operator: Manufacturer:
The Norwegian EPD Foundation Sto Scandinavia AB
Post Box 5250 Majorstuen, 0303 Oslo, Norway Gesällgatan 6
Phone: +47 977 22 020 SE-582 77 Linköping, Sweden
web: www.epd-norge.no
Declaration number: Place of production:
Linköping
NEPD-8924-8584
Gesällgatan 6
SE-582 77 Linköping, Sweden
This declaration is based on Product Category Rules: Management system:
CEN Standard EN 15804:2012+A2:2019 serves as core PCR ISO 14001; ISO 50001; ISO 9001
NPCR 009:2021 Part B for Technical - Chemical products for building
and construction industry
Statement of liability: Organisation no:
The owner of the declaration shall be liable for the underlying DE142834082
information and evidence. EPD Norway shall not be liable with respect
to manufacturer information, life cycle assessment data and
evidences.​
Declared unit: Issue date:
1 kg Self-levelling compounds StoCrete CS 730 and StoCrete CS 735
04.02.2025
Declared unit with option: Valid to:
A1,A2,A3,A4,A5,C1,C2,C3,C4,D
04.02.2030
Year of study:
2023
Functional unit: Comparability:
EPD of construction products may not be comparable if they not
comply with EN 15804 and seen in a building context.
General information on verification of EPD from EPD tools: Development and verification of EPD:
Independent verification of data, other environmental information The declaration is created using EPD tool lca.tools ver EPD2022.03,
and the declaration according to ISO 14025:2010, § 8.1.3 and § 8.1.4. developed by LCA.no. The EPD tool is integrated in the company's
Verification of each EPD is made according to EPD-Norway’s management system, and has been approved by EPD Norway.
guidelines for verification and approval requiring that tools are i) NEPDT143
integrated into the company's environmental management system, ii)
the procedures for use of the EPD tool are approved by EPD-Norway, Developer of EPD: Angelica Hultin
and iii) the process is reviewed annually by an independent third
Reviewer of company-specific input data and EPD: Karin Bromoe
party verifier. See Appendix G of EPD-Norway's General Programme
Instructions for further information on EPD tools
Verification of EPD tool: Approved:
Independent third party verification of the EPD tool, background data
and test-EPD in accordance with EPDNorway's procedures and
guidelines for verification and approval of EPD tools. NEPDT73
Third party verifier:
Linda Høibye, Life Cycle Assessment Consulting
(no signature required)
2 / 12
Product
Product description:
The EPD covers the following products:
* StoCrete CS 730
* StoCrete CS 735
The values are based on StoCrete 730, which has the highest GWP values of the two products.
Both products are within ± 10% for the GWP-total indicator. The product with the highest GWP has been used as a basis for this EPD.
StoCrete CS 730 and StoCrete CS 735 are indoor cementitious self-leveling compounds for medium pressure load. StoCrete CS 730 and StoCrete
CS 735 are produced as a dry powder and mixed with water at the building site.
They are used in homes, offices and public buildings.
Product specification
The contents of StoCrete CS 730 and StoCrete CS 735 are described in the table below:
Materials Value Unit
Cement 10-15 %
Additives <1 %
Pigments and fillers 70-80 %
Packaging 1-5 %
Binder 5-10 %
Technical data:
• Pumpable and self-levelling
• For medium loads
• Meets conditions according to EN 13813
For more information, see the technical data sheet at www.sto.se.
Market:
The main market is the Nordic countries.
Reference service life, product
50
A reference service life (RSL) as per ISO 15686-1, -2, - 7, and -8 is not declared. In this LCA an RSL of 50 years has been declared, equal to the
useful life of the building (according to standard 15804+A2), since the product is incorporated in the building structure.
Reference service life, building
50
LCA: Calculation rules
Declared unit:
1 kg Self-levelling compounds StoCrete CS 730 and StoCrete CS 735
Cut-off criteria:
All major raw materials and all the essential energy is included. The production processes for raw materials and energy flows with very small
amounts (less than 1%) are not included. These cut-off criteria do not​ apply for hazardous materials and substances.
Allocation:
The allocation is made in accordance with the provisions of EN 15804. Incoming energy and water and waste production in-house is allocated
equally among all products through mass allocation. Effects of primary production of recycled materials is allocated to the main product in which
the material was used. The recycling process and transportation of the material is allocated to this analysis.
Data quality:
Specific data for the product composition are provided by the manufacturer. The data represent the production of the declared product and were
collected for EPD development in the year of study. Background data is based on EPDs according to EN 15804 and different LCA databases. The
data quality of the raw materials in A1 is presented in the table below.
3 / 12
Materials Source Data quality Year
Additives CEPE RM Database v3.0 Database 2016
Additives Ecoinvent 3.6 Database 2019
Aggregate ecoinvent 3.6 Database 2019
Binders and Resins CEPE RM Database v3.0 Database 2016
Cement ecoinvent 3.6 Database 2019
Chemical ecoinvent 3.6 Database 2019
Packaging - Paper ecoinvent 3.6 Database 2019
Packaging - Plastic ecoinvent 3.6 Database 2019
Packaging - Wood Modified ecoinvent 3.6 Database 2019
Pigments and Fillers CEPE RM Database v3.0 Database 2016
SCM ecoinvent 3.6 Database 2019
4 / 12
System boundaries (X=included, MND=module not declared, MNR=module not relevant)
Construction Beyond the system
Product stage Use stage End of life stage
installation stage boundaries
A1 A2 A3 A4 A5 B1 B2 B3 B4 B5 B6 B7 C1 C2 C3 C4 D
X X X X X MND MND MND MND MND MND MND X X X X X
System boundary:
The approach is “cradle-to-grave” but with exclusion of the use stage (B1-B7). Stage B1-B7 is not applicable for this cement based product. This
product does not require any actions or maintenance operations during the use stages. The following modules have been considered:
A1, A2, A3 (Product stages): Extraction and transport of raw materials, including packaging, and manufacturing process
A4 (Transport to market): Transportation from manufacturing plant to customer
A5 (Assembly): Installation at construction site
C1, C2, C3, C4 (End of life stages): Deconstruction, demolition, transport to waste processing, waste processing for reuse, recovery and/or recycling
and disposal
D (Benefits and loads beyond the system boundaries): Reuse/recovery/recycling potential
Additional technical information:
The waste code for unused product is 17 09 03* Other construction and demolition wastes (including mixed waste) containing hazardous
substances. See MSDS section 13.
Hardened product is not classified as dangerous waste.
waR slairetam tropsnarT gnirutcafunaM tropsnarT ylbmessA e​sU ecnanetniaM riapeR tnemecalpeR tnemhsibrufeR lanoitarepO ygrene esu lanoitarepO esu retaw -eD noitcurtsnoc noitilomed tropsnarT etsaW gnissecorp lasopsiD -yrevoceR-esueR laitnetop-gnilcyceR
5 / 12
LCA: Scenarios and additional technical information
The following information describe the scenarios in the different modules of the EPD.
A4 (Transport to market/building site): Most of our transports are from the production site in Linköping to customers in Stockholm. We have
therefore taken this distance as an average. This gives the value of 200 km. Transport method is Lorries (Trucks) in the tonnage range 16-32 t.
A5 (Installation): The product is used in a wet state, it is mixed with water at the building site according to specifications in the technical data sheet.
Application of the mortar is either by hand or with a mixer pump together with a plaster gun. Electricity for application with machine has been
taken into account in this LCA. Outputs are small amounts of waste from the product itself (assumed to be less than 5%) and waste from
packaging materials.
C1 (De-construction, demolition): The product is demolished together with the concrete structure. In this LCA we have assumed a scenario where
the product is demolished together with the whole building/structure.
C2 (Transport end of life): This stage includes the transportation effects of demolished waste to a waste processing area. The distance between the
demolishing area and a waste processing area is assumed to be quite short (less than 100 km). The distance varies depending on the type of
waste processing.
C3 (Waste processing): In this LCA we have assumed a typical waste scenario for concrete waste (cement-based products) that estimates that 10%
of the product is recycled. The product can be used as filling masses in for instance road construction. The most part is assumed to be put on
landfill (90%).
C4 (Final disposal): Mineral construction waste is categorized as non-hazardous waste. The product can therefore be used in landfills. The degree
of landfill and possibility to recycle the mineral waste is taken into account when disposing of the product. The degree of landfill is assumed to be
90% and the rest is assumed to be recycled.
D (Environmental costs and benefits of recycling and reuse): It is preferable if mineral construction waste can be recycled, since this would save
resources such as raw materials and also save energy during production. 10% of the product is estimated to be recycled.
Capacity utilisation Value
Transport from production place to user (A4) Distance (km) Fuel/Energy Consumption Unit
(incl. return) % (Liter/tonne)
Truck, 16-32 tonnes, EURO 6 (kgkm) 36,7 % 200 0,043 l/tkm 8,60
Assembly (A5) Unit Value
Waste, packaging, pallet, EUR wooden pallet,
kg 0,010
reusable, average treatment (kg)
Material loss, including waste treatment (psc) Units/DU 0,050
Tap water (kg) kg/DU 0,18
Waste, bag, 84% paper and 16% LDPE, to average
kg 0,0019
treatment (kg)
Waste, packaging, plastic film (LDPE), to average
kg 0,000072
treatment (kg)
Electricity, Nordic (kWh) kWh/DU 0,0027
De-construction demolition (C1) Unit Value
Demolition of building per kg of cement-based
kg/DU 1,000000000
product, C1 (kg)
Capacity utilisation Value
Transport to waste processing (C2) Distance (km) Fuel/Energy Consumption Unit
(incl. return) % (Liter/tonne)
Truck, 16-32 tonnes, EURO 6 (kgkm) 36,7 % 100 0,043 l/tkm 4,30
Waste processing (C3) Unit Value
Waste treatment of cement-based product after
kg 0,10
demolition (kg) - C3, 100% to recycling
Disposal (C4) Unit Value
Waste, inert waste, to landfill (kg) kg 0,90
Benefits and loads beyond the system
Unit Value
boundaries (D)
Substitution of thermal energy, district heating
MJ 0,0055
(MJ)
Substitution of electricity (MJ) MJ 0,00036
Substitution of primary aggregates with crushed
kg 0,10
recycled cement-based products (kg)
6 / 12
LCA: Results
The LCA results are presented below for the declared unit defined on page 2 of the EPD document.
Environmental impact
Indicator Unit A1 A2 A3 A4 A5 C1 C2 C3 C4 D
GWP-total
kg CO2 -
2,73E-01 1,13E-01 3,94E-04 3,29E-02 3,97E-02 0,00E+00 1,65E-02 7,20E-05 7,39E-03 -2,67E-04
eq
GWP-fossil
kg CO2 -
2,91E-01 1,13E-01 3,63E-04 3,29E-02 2,41E-02 0,00E+00 1,64E-02 7,10E-05 7,38E-03 -2,61E-04
eq
GWP-biogenic
kg CO2 -
-1,84E-02 3,67E-05 2,44E-05 1,36E-05 1,55E-02 0,00E+00 6,81E-06 6,13E-07 8,62E-06 -4,63E-06
eq
GWP-luluc
kg CO2 -
1,11E-04 5,71E-05 6,13E-06 1,17E-05 2,97E-05 0,00E+00 5,85E-06 9,83E-08 1,81E-06 -1,26E-06
eq
kg
ODP CFC11 - 8,22E-09 2,44E-08 6,80E-11 7,45E-09 2,37E-09 0,00E+00 3,73E-09 1,40E-11 2,80E-09 -2,34E-06
eq
mol H+
AP 8,39E-04 2,45E-03 2,01E-06 9,45E-05 1,70E-04 0,00E+00 4,73E-05 5,75E-07 6,57E-05 -2,32E-06
-eq
EP-FreshWater kg P -eq 9,32E-06 6,13E-07 3,16E-08 2,63E-07 5,44E-07 0,00E+00 1,31E-07 4,49E-09 8,37E-08 -8,94E-09
EP-Marine kg N -eq 1,75E-04 6,07E-04 6,06E-07 1,87E-05 4,12E-05 0,00E+00 9,35E-06 1,68E-07 2,44E-05 -8,01E-07
mol N -
EP-Terrestial 1,93E-03 6,75E-03 7,35E-06 2,09E-04 4,50E-04 0,00E+00 1,05E-04 1,94E-06 2,69E-04 -9,33E-06
eq
kg
POCP NMVOC 5,35E-04 1,79E-03 1,64E-06 8,01E-05 1,23E-04 0,00E+00 4,01E-05 5,20E-07 7,71E-05 -2,47E-06
-eq
ADP- kg Sb-
2,00E-06 1,25E-06 7,53E-09 9,09E-07 1,89E-07 0,00E+00 4,54E-07 9,01E-10 6,65E-08 -2,06E-08
minerals&metals1 eq
ADP-fossil1 MJ 3,03E+00 1,60E+00 1,28E-02 4,97E-01 2,90E-01 0,00E+00 2,49E-01 2,21E-03 2,03E-01 -4,33E-03
WDP1 m3 1,60E+01 7,15E-01 1,08E+00 4,81E-01 1,79E+00 0,00E+00 2,41E-01 2,43E-01 1,25E+00 -1,87E-01
GWP-total = Global Warming Potential total; GWP-fossil = Global Warming Potential fossil fuels; GWP-biogenic = Global Warming Potential biogenic; GWP-luluc =
Global Warming Potential land use and land use change; ODP = Depletion potential of the stratospheric ozone layer; AP = Acidification potential, Accumulated
Exceedance; EP-freshwater = Eutrophication potential, fraction of nutrients reaching freshwater end compartment: EP-marine = Eutrophication potential, fraction of
nutrients reaching marine end compartment; EP-terrestrial = Eutrophication potential, Accumulated Exceedance; POCP = Formation potential of tropospheric ozone;
ADP-minerals&metals = Abiotic depletion potential for non-fossil resources; ADP-fossil = Abiotic depletion for fossil resources potential; WDP = Water (user)
deprivation potential, deprivation-weighted water consumption
"Reading example: 9,0 E-03 = 9,0*10-3 = 0,009"
*INA Indicator Not Assessed
1. The results of this environmental impact indicator shall be used with care as the uncertainties on these results are high or as there is limited experienced with the
indicator
Remarks to environmental impacts
7 / 12
Additional environmental impact indicators
Indicator Unit A1 A2 A3 A4 A5 C1 C2 C3 C4 D
PM Disease incidence 1,21E-06 5,84E-09 1,25E-07 2,01E-09 6,72E-08 0,00E+00 1,01E-09 9,00E-12 1,40E-09 -6,00E-11
IRP2 kgBq U235 -eq 1,59E+01 6,92E-03 3,67E-04 2,17E-03 7,90E-01 0,00E+00 1,09E-03 3,70E-05 9,27E-04 -3,85E-05
ETP-fw1 CTUe 1,29E+00 1,02E+00 5,91E-03 3,69E-01 1,60E-01 0,00E+00 1,84E-01 1,56E-03 1,11E-01 -6,48E-03
HTP-c1 CTUh 1,30E-10 0,00E+00 0,00E+00 0,00E+00 7,00E-12 0,00E+00 0,00E+00 0,00E+00 5,00E-12 0,00E+00
HTP-nc1 CTUh 6,07E-09 1,13E-09 4,00E-12 4,03E-10 4,11E-10 0,00E+00 2,01E-10 1,00E-12 8,00E-11 -7,00E-12
SQP1 dimensionless 6,12E-01 9,05E-01 4,94E-03 3,48E-01 1,51E-01 0,00E+00 1,74E-01 1,25E-03 7,82E-01 5,72E-03
PM = Particulate Matter emissions; IRP = Ionizing radiation – human health; ETP-fw = Eco toxicity – freshwater; HTP-c = Human toxicity – cancer effects; HTP-nc =
Human toxicity – non cancer effects; SQP = Potential Soil Quality Index (dimensionless)
"Reading example: 9,0 E-03 = 9,0*10-3 = 0,009"
*INA Indicator Not Assessed
1. The results of this environmental impact indicator shall be used with care as the uncertainties on these results are high or as there is limited experienced with the
indicator
2. This impact category deals mainly with the eventual impact of low dose ionizing radiation on human health of the nuclear fuel cycle. It does not consider effects due
to possible nuclear accidents, occupational exposure nor due to radioactive waste disposal in underground facilities. Potential ionizing radiation from the soil, from
radon and from some construction materials is also not measured by this indicator.
8 / 12
Resource use
Indicator Unit A1 A2 A3 A4 A5 C1 C2 C3 C4 D
PERE MJ 6,01E-01 1,45E-02 6,58E-03 7,12E-03 4,19E-02 0,00E+00 3,56E-03 1,14E-03 7,27E-03 -3,74E-03
PERM MJ 1,70E-01 0,00E+00 0,00E+00 0,00E+00 -1,61E-01 0,00E+00 0,00E+00 0,00E+00 0,00E+00 0,00E+00
PERT MJ 7,71E-01 1,45E-02 6,58E-03 7,12E-03 -1,19E-01 0,00E+00 3,56E-03 1,14E-03 7,27E-03 -3,74E-03
PENRE MJ 3,16E+00 1,60E+00 1,30E-02 4,97E-01 2,97E-01 0,00E+00 2,49E-01 2,21E-03 2,03E-01 -4,55E-03
PENRM MJ 3,84E-01 0,00E+00 0,00E+00 0,00E+00 -1,52E-02 0,00E+00 0,00E+00 -3,68E-01 0,00E+00 0,00E+00
PENRT MJ 3,54E+00 1,60E+00 1,30E-02 4,97E-01 2,81E-01 0,00E+00 2,49E-01 -3,66E-01 2,03E-01 -4,55E-03
SM kg 0,00E+00 0,00E+00 0,00E+00 0,00E+00 0,00E+00 0,00E+00 0,00E+00 0,00E+00 0,00E+00 0,00E+00
RSF MJ 3,33E-03 4,54E-04 2,01E-05 2,55E-04 3,28E-04 0,00E+00 1,27E-04 0,00E+00 1,51E-04 -1,90E-05
NRSF MJ 2,39E-04 1,03E-03 6,34E-05 9,11E-04 1,70E-04 0,00E+00 4,55E-04 0,00E+00 3,26E-04 -1,87E-04
FW m3 2,57E-01 1,23E-04 1,21E-05 5,32E-05 1,31E-02 0,00E+00 2,66E-05 3,78E-06 2,50E-04 -1,46E-04
PERE = Use of renewable primary energy excluding renewable primary energy resources used as raw materials; PERM = Use of renewable primary energy resources used
as raw materials; PERT = Total use of renewable primary energy resources; PENRE = Use of non renewable primary energy excluding non-renewable primary energy
resources used as raw materials; PENRM = Use of non renewable primary energy resources used as raw materials; PENRT = Total use of non renewable primary energy
resources; SM = Use of secondary materials; RSF = Use of renewable secondary fuels; NRSF = Use of non-renewable secondary fuels; FW = Net use of fresh water
"Reading example: 9,0 E-03 = 9,0*10-3 = 0,009"
*INA Indicator Not Assessed
9 / 12
End of life - Waste
Indicator Unit A1 A2 A3 A4 A5 C1 C2 C3 C4 D
HWD kg 4,51E-04 7,46E-05 5,32E-05 2,57E-05 3,13E-05 0,00E+00 1,28E-05 2,20E-07 0,00E+00 -9,55E-07
NHWD kg 8,09E-01 6,18E-02 6,19E-05 2,42E-02 9,30E-02 0,00E+00 1,21E-02 6,96E-06 9,00E-01 -3,92E-05
RWD kg 9,53E-06 1,10E-05 8,39E-07 3,39E-06 1,42E-06 0,00E+00 1,69E-06 2,33E-08 0,00E+00 -3,31E-08
HWD = Hazardous waste disposed; NHWD = Non-hazardous waste disposed; RWD = Radioactive waste disposed
"Reading example: 9,0 E-03 = 9,0*10-3 = 0,009"
*INA Indicator Not Assessed
End of life - Output flow
Indicator Unit A1 A2 A3 A4 A5 C1 C2 C3 C4 D
CRU kg 0,00E+00 0,00E+00 0,00E+00 0,00E+00 1,01E-02 0,00E+00 0,00E+00 0,00E+00 0,00E+00 0,00E+00
MFR kg 0,00E+00 0,00E+00 1,66E-02 0,00E+00 5,88E-03 0,00E+00 0,00E+00 1,00E-01 0,00E+00 0,00E+00
MER kg 0,00E+00 0,00E+00 1,00E-05 0,00E+00 1,91E-03 0,00E+00 0,00E+00 0,00E+00 0,00E+00 0,00E+00
EEE MJ 0,00E+00 0,00E+00 1,47E-05 0,00E+00 1,19E-03 0,00E+00 0,00E+00 0,00E+00 0,00E+00 0,00E+00
EET MJ 0,00E+00 0,00E+00 2,23E-04 0,00E+00 1,80E-02 0,00E+00 0,00E+00 0,00E+00 0,00E+00 0,00E+00
CRU = Components for re-use; MFR = Materials for recycling; MER = Materials for energy recovery; EEE = Exported energy electrical; EET = Exported energy thermal
"Reading example: 9,0 E-03 = 9,0*10-3 = 0,009"
*INA Indicator Not Assessed
Biogenic Carbon Content
Indicator Unit At the factory gate
Biogenic carbon content in product kg C 0,00E+00
Biogenic carbon content in accompanying packaging kg C 5,14E-03
Note: 1 kg biogenic carbon is equivalent to 44/12 kg CO2
10 / 12
Additional requirements
Greenhouse gas emissions from the use of electricity in the manufacturing phase
National production mix from import, low voltage (production of transmission lines, in addition to direct emissions and losses in grid) of applied
electricity for the manufacturing process (A3).
Electricity mix Source Amount Unit
Electricity, Sweden (kWh) ecoinvent 3.6 54,94 g CO2-eq/kWh
Dangerous substances
The product contains no substances given by the REACH Candidate list.
Indoor environment
Emission measurements according to ISO 16000-9:2024 (Indoor air - Part 9: Determination of the emission of volatile organic compounds from
samples of building products and furnishing - Emission test chamber method), after 28 days regarding volatile organic compounds (VOC and
VVOC/SVOC), carcinogenic substances (VOC-substances, EU Regulation No 1272/2008
Annex VI, cat 1A and 1B) and aldehydes.
Test results (µg/m³)
StoCrete CS 730:
TVOC: <10; CMR 1A+1B: <1; Single VOC: < EU-LCI; Formaldehyde: 67; R value: <1
StoCrete CS 735:
TVOC: 26; CMR 1A+1B: <1; Single VOC: < EU-LCI; Formaldehyde: 13; R value: <1
Additional Environmental Information
Additional environmental impact indicators required in NPCR Part A for construction products
Indicator Unit A1 A2 A3 A4 A5 C1 C2 C3 C4 D
GWPIOBC kg CO2 -eq 2,91E-01 1,13E-01 3,71E-04 3,29E-02 2,43E-02 0,00E+00 1,65E-02 7,11E-05 7,39E-03 -2,78E-04
GWP-IOBC: Global warming potential calculated according to the principle of instantaneous oxidation. In order to increase the transparency of biogenic carbon​
contribution to climate impact, the indicator GWP-IOBC is required as it declares climate impacts calculated according to the principle of instantaneous oxidation.​
GWP-IOBC is also referred to as GWP-GHG in context to Swedish public procurement legislation.
11 / 12
Bibliography
ISO 14025:2010 Environmental labels and declarations - Type III environmental declarations - Principles and procedures.
ISO 14044:2006 Environmental management - Life cycle assessment - Requirements and guidelines.
EN 15804:2012+A2:2019 Environmental product declaration - Core rules for the product category of construction products.
ISO 21930:2017 Sustainability in buildings and civil engineering works - Core rules for environmental product declarations of construction
products.
ecoinvent v3, (2019) Allocation, cut-off by classification, Swiss Centre of Life Cycle Inventories.
Iversen et al., (2021) eEPD v2021.09 Background information for EPD generator tool system verification, LCA.no Report number: 07.21
Ruttenborg, M. and Iversen, O.M.K., (2023) EPD generator for NPCR009:2021, Part B for Technical - Chemical products, Background information
for EPD generator application and LCA data, LCA.no report number: 05.23.
NPCR Part A: Construction products and services. Ver. 2.0, 24.03.2021 EPD Norway.
NPCR 009 Part B for Technical - Chemical products for building and construction industry, Ver. 3.0, 06.10.2021, EPD Norway.
RISE Research Institutes of Sweden AB, Emission measurements after 28 days, Ref. O100785-1290900-3
RISE Research Institutes of Sweden AB, Emission measurements after 28 days, Ref. O100785-1290900-4
Program operator and publisher Phone: +47 977 22 020
The Norwegian EPD Foundation e-mail: post@epd-norge.no
Post Box 5250 Majorstuen, 0303 Oslo, Norway web: www.epd-norge.no
Owner of the declaration: Phone: +49 7744571010
Sto SE & Co. KGaA e-mail: l.kaltenbach@sto.com
Ehrenbachstraße 1, 79780 Stühlingen, Germany web: https://www.sto.com/
Author of the Life Cycle Assessment Phone: +47 916 50 916
LCA.no AS e-mail: post@lca.no
Dokka 6A, 1671 Kråkerøy, Norway web: www.lca.no
Developer of EPD generator Phone: +47 916 50 916
LCA.no AS e-mail: post@lca.no
Dokka 6A, 1671 Kråkerøy, Norway web: www.lca.no
ECO Platform web: www.eco-platform.org
ECO Portal web: ECO Portal
12 / 12
