ENVIRONMENTAL PRODUCT DECLARATION
as per ISO 14025 and EN 15804+A2
Owner of the Declaration dormakaba International Holding GmbH
Publisher Institut Bauen und Umwelt e.V. (IBU)
Programme holder Institut Bauen und Umwelt e.V. (IBU)
Declaration number EPD-DOR-20240051-CBA1-EN
Issue date 22.03.2024
Valid to 21.03.2029
Safe Lock Auditcon
dormakaba
www.ibu-epd.com | https://epd-online.com
General Information
dormakaba Safe Lock Auditcon
Programme holder Owner of the declaration
IBU – Institut Bauen und Umwelt e.V. dormakaba International Holding GmbH
Hegelplatz 1 DORMA Platz 1
10117 Berlin 58256 Ennepetal
Germany Germany
Declaration number Declared product / declared unit
EPD-DOR-20240051-CBA1-EN 1 piece of the product: Auditcon consisting of the following items:
• Auditcon lock 552
• Case
• Bolt
• Cover
• Keypad
• Card
• Product packaging
This declaration is based on the product category rules: Scope:
Electronic and physical Access Control Systems, 01.08.2021 This Environmental Product Declaration refers to a specific safe lock
(PCR checked and approved by the SVR) Auditcon manufactured by dormakaba. The production site is located in
Nogales (Mexico).
Issue date The data represents the year 2024.
The owner of the declaration shall be liable for the underlying information
22.03.2024
and evidence; the IBU shall not be liable with respect to manufacturer
information, life cycle assessment data and evidences.
Valid to
The EPD was created according to the specifications of EN 15804+A2. In
21.03.2029 the following, the standard will be simplified as EN 15804.
Verification
The standard EN 15804 serves as the core PCR
Independent verification of the declaration and data according to ISO
14025:2011
internally X externally
Dipl.-Ing. Hans Peters
(Chairman of Institut Bauen und Umwelt e.V.)
Florian Pronold Matthias Klingler,
(Managing Director Institut Bauen und Umwelt e.V.) (Independent verifier)
1 Environmental Product Declaration - dormakaba - Safe Lock Auditcon
Product
The product with respect to its characteristics is in accordance
Product description/Product definition with the relevant technical provisions (no CE-marking):
The safe lock series Audicon protects from unauthorized
• VDS 2344
access. The series is totally self-powered, using the PowerStar
• VDS 2396
Technology. Auditcon offers the advantages and convenience of
• EN 1300
true stand-alone electronic safe access. It was developed to
• UL 2058
address the security requirements of a broad range of retail,
commercial and industrial markets.
Base materials/Ancillary materials
For the safe lock Auditcon the standards which can be applied
The major material composition including the packaging of the
are the following:
product is listed below:
• VDS 2344 Name Value Unit
• VDS 2396
Plastics 43 %
• EN 1300
Paper 20 %
• UL 2058
• 2011/65/EU (RoHS) Steel 16 %
Zinc 12 %
The CE marking takes into account the proof of conformity Electronics 8 %
with the respective harmonised standards based on the legal
Brass 1 %
provisions above.
The product includes partial articles which contain substances
Application listed in the Candidate List of REACH Regulation
The Auditcon family of electronic locks addresses the 1907/2006/EC (date: 23.01.2024) exceeding 0.1 percentage by
security requirements of a broad range of financial, retail, mass: no
commercial and industrial markets.
The Candidate List can be found on the ECHA website
Technical Data address: https:echa.europa.eu/de/home.
The safe lock Auditcon has following technical properties:
Name Value Unit
Reference service life
Power Unit n.a. Solenoid driven
The reference service life of the safe lock Auditcon amounts to
Power Source n.a. Self powered PowerStar® Technology
7 years, depending on the application and frequency of use.
Battery Assist 9 V Alkaline
For repairs and renewals, suitable spare parts are available.
The safe lock is tested and certified to UL 2058, meaning they
are designed to withstand a minimum of 25.000 cycles.
LCA: Calculation rules
building; including provision of all materials, products and
Declared Unit energy, as well as waste processing up to the end-of-waste
state or disposal of final residues during the construction
The declared unit is 1 piece of the product: Auditcon including process stage.
packaging
Name Value Unit End-of-life stage– Modules C1-C4 and D
The end-of-life stage includes: — C1, de-construction,
Declared unit 1 piece/product
demolition: — C2, transport to waste processing; — C3, waste
Mass of declared Product 0.949 kg
processing for reuse, recovery and/or recycling; — C4,
disposal; including provision and all transport, provision of all
materials, products and related energy and water use. Module
System boundary
D (Benefits and loads beyond the system boundary) includes:
The type of EPD is: cradle to gate with options, modules C1– — D, recycling potentials, expressed as net impacts and
C4, and module D (A1–A3 + C + D and additional modules: benefits.
A4+ A5)
Geographic Representativeness
Production - Module A1-A3 Land or region, in which the declared product system is
The product stage includes: — A1, raw material extraction, manufactured, used or handled at the end of the product´s
processing and mechanical treatments, processing of lifespan: Global
secondary material input (e.g. recycling processes), — A2,
transport to the manufacturer, — A3, manufacturing and
assembly including provision of all materials, products and Comparability
energy, as well as waste processing up to the end-of-waste Basically, a comparison or an evaluation of EPD data is only
state. possible if all the data sets to be compared were created
according to EN 15804 and the building context, respectively
Construction stage - Modules A4-A5 the product-specific characteristics of performance, are taken
The construction process stage includes: into account. Background database: GaBi, SP40.
— A4, transport to the building site; — A5, installation into the
2 Environmental Product Declaration - dormakaba - Safe Lock Auditcon
LCA: Scenarios and additional technical information
Characteristic product properties of biogenic carbon
Reference service life
Name Value Unit
Information on describing the biogenic carbon content at
Life Span according to the manufacturer 7 a
factory gate
Name ValueUnit End of life (C1-C4)
kg C1: The product dismantling from the building is done manually
Biogenic carbon content in product 0.02
C without environmental burden.
Biogenic carbon content in accompanying kg C2: Transport to waste management is 50 km.
0.05
packaging C Name Value Unit
Note: 1 kg of biogenic carbon is equivalent to 44/12 kg of CO . Collected separately waste type waste type 0.815 kg
2
Recycling 0.341 kg
Energy recovery 0.404 kg
Landfilling 0.07 kg
The product is disassembled in a recycling process. Material
Transport to the building site (A4)
recycling is then assumed for metals and electronics. The
Name Value Unit plastic components are assumed to be incinerated with energy
Litres of fuel 0.00276 l/100km recovery. Minor proportions of residues arising from the
Transport distance 100 km recycling process are landfilled. Region for the End of Life is:
Global.
Capacity utilisation (including empty runs) 55 %
The product is transported via truck. The product is stored in
Reuse, recovery and/or recycling potentials (D), relevant
the dormakaba plant in Mexico. The main distribution regions
scenario information
are North- and South America. In order to allow scaling to a
Name Value Unit
specific point of installation 100 km are declared.
Recycling 100 %
Installation into the building (A5) The collection rate is 100 %.
Name Value Unit
Waste packaging (paper and plastic) 0,134 kg
3 Environmental Product Declaration - dormakaba - Safe Lock Auditcon
LCA: Results
DESCRIPTION OF THE SYSTEM BOUNDARY (X = INCLUDED IN LCA; MND = MODULE OR INDICATOR NOT DECLARED; MNR
= MODULE NOT RELEVANT)
Benefits and
Construction loads beyond
Product stage Use stage End of life stage
process stage the system
boundaries
la ire ta m w a Ry lp p u s tro p s n a rT g n iru tc a fu n a M e h t m o rf tro p s n a rTe tis e h t o t e ta g y lb m e s s A e s U e c n a n e tn ia M ria p e R tn e m e c a lp e R tn e m h s ib ru fe R y g re n e la n o ita re p Oe s u re ta w la n o ita re p Oe s u n o itc u rts n o c -e Dn o itilo m e d tro p s n a rT g n is s e c o rp e ts a W la s o p s iD -e s u e R-y re v o c e R-g n ilc y c e Rla itn e to p
A1 A2 A3 A4 A5 B1 B2 B3 B4 B5 B6 B7 C1 C2 C3 C4 D
X X X X X MND MND MNR MNR MNR MND MND X X X X X
RESULTS OF THE LCA - ENVIRONMENTAL IMPACT according to EN 15804+A2: 1 piece Auditcon
Parameter Unit A1-A3 A4 A5 C1 C2 C3 C4 D
GWP-total kg CO 2 eq 5.03E+00 8E-03 1.91E-01 0 4E-03 1.14E+00 1E-03 -1.04E+00
GWP-fossil kg CO 2 eq 5.24E+00 8E-03 6E-03 0 4E-03 1.03E+00 1E-03 -1.04E+00
GWP-biogenic kg CO 2 eq -2.14E-01 3.67E-04 1.85E-01 0 1.65E-04 1.08E-01 3.62E-06 -2E-03
GWP-luluc kg CO 2 eq 5.28E-03 1.89E-07 3.19E-06 0 8.47E-08 5.91E-05 3.04E-06 -6.41E-04
ODP kg CFC11 eq 2.09E-10 8.38E-19 3.48E-17 0 3.76E-19 5.31E-16 3.92E-18 -2.71E-14
AP mol H+ eq 3.79E-02 7.94E-06 5.34E-05 0 3.56E-06 1.98E-04 7.59E-06 -3E-03
EP-freshwater kg P eq 2.15E-05 1.7E-09 6.79E-09 0 7.62E-10 8.46E-08 1.82E-09 -1.81E-06
EP-marine kg N eq 5.66E-03 2.53E-06 1.93E-05 0 1.13E-06 4.63E-05 1.95E-06 -5.11E-04
EP-terrestrial mol N eq 6E-02 2.81E-05 2.4E-04 0 1.26E-05 9.06E-04 2.15E-05 -5E-03
kg NMVOC
POCP 1.67E-02 7.14E-06 5.11E-05 0 3.21E-06 1.28E-04 5.91E-06 -2E-03
eq
ADPE kg Sb eq 2E-03 2.38E-10 5.49E-10 0 1.07E-10 7.31E-09 9.5E-11 -1.77E-04
ADPF MJ 8.08E+01 1.13E-01 6.1E-02 0 5E-02 4.99E-01 1.4E-02 -1.59E+01
m3 world eq
WDP 1.07E+00 1.56E-05 2.4E-02 0 6.98E-06 1.16E-01 1.11E-04 -1.4E-01
deprived
GWP = Global warming potential; ODP = Depletion potential of the stratospheric ozone layer; AP = Acidification potential of land and water; EP =
Eutrophication potential; POCP = Formation potential of tropospheric ozone photochemical oxidants; ADPE = Abiotic depletion potential for non-fossil
resources; ADPF = Abiotic depletion potential for fossil resources; WDP = Water (user) deprivation potential)
RESULTS OF THE LCA - INDICATORS TO DESCRIBE RESOURCE USE according to EN 15804+A2: 1 piece Auditcon
Parameter Unit A1-A3 A4 A5 C1 C2 C3 C4 D
PERE MJ 1.4E+01 3.55E-04 1.62E+00 0 1.59E-04 8.51E-01 2E-03 -3.02E+00
PERM MJ 2.33E+00 0 -1.61E+00 0 0 -7.23E-01 0 0
PERT MJ 1.63E+01 3.55E-04 1.1E-02 0 1.59E-04 1.28E-01 2E-03 -3.02E+00
PENRE MJ 6.5E+01 1.13E-01 8E-02 0 5.1E-02 1.63E+01 1.4E-02 -1.59E+01
PENRM MJ 1.58E+01 0 -2E-02 0 0 -1.58E+01 0 0
PENRT MJ 8.08E+01 1.13E-01 6.1E-02 0 5.1E-02 5E-01 1.4E-02 -1.59E+01
SM kg 1.28E-01 0 0 0 0 0 0 0
RSF MJ 0 0 0 0 0 0 0 0
NRSF MJ 0 0 0 0 0 0 0 0
FW m3 2.9E-02 6.36E-07 5.57E-04 0 2.86E-07 3E-03 3.5E-06 -5E-03
PERE = Use of renewable primary energy excluding renewable primary energy resources used as raw materials; PERM = Use of renewable primary
energy resources used as raw materials; PERT = Total use of renewable primary energy resources; PENRE = Use of non-renewable primary energy
excluding non-renewable primary energy resources used as raw materials; PENRM = Use of non-renewable primary energy resources used as raw
materials; PENRT = Total use of non-renewable primary energy resources; SM = Use of secondary material; RSF = Use of renewable secondary fuels;
NRSF = Use of non-renewable secondary fuels; FW = Use of net fresh water
RESULTS OF THE LCA – WASTE CATEGORIES AND OUTPUT FLOWS according to EN 15804+A2:
1 piece Auditcon
Parameter Unit A1-A3 A4 A5 C1 C2 C3 C4 D
HWD kg 1.75E-06 1.09E-11 9.04E-11 0 4.9E-12 1.83E-09 2.12E-10 -2.16E-07
NHWD kg 2.06E-01 1.15E-05 6E-03 0 5.17E-06 1.07E-01 7E-02 1.6E-02
RWD kg 2.06E-03 1.21E-07 3.17E-06 0 5.42E-08 1.9E-05 1.58E-07 -9.42E-04
CRU kg 0 0 0 0 0 0 0 0
MFR kg 0 0 0 0 0 3.18E-01 0 0
MER kg 0 0 0 0 0 0 0 0
EEE MJ 0 0 2.9E-01 0 0 2.11E+00 0 0
EET MJ 0 0 5.26E-01 0 0 4.77E+00 0 0
4 Environmental Product Declaration - dormakaba - Safe Lock Auditcon
HWD = Hazardous waste disposed; NHWD = Non-hazardous waste disposed; RWD = Radioactive waste disposed; CRU = Components for re-use;
MFR = Materials for recycling; MER = Materials for energy recovery; EEE = Exported electrical energy; EET = Exported thermal energy
RESULTS OF THE LCA – additional impact categories according to EN 15804+A2-optional:
1 piece Auditcon
Parameter Unit A1-A3 A4 A5 C1 C2 C3 C4 D
Disease
PM 3.46E-07 4.17E-11 2.97E-10 0 1.87E-11 2.41E-09 9.39E-11 -3.45E-08
incidence
IR kBq U235 eq 1.79E-01 1.73E-05 4.9E-04 0 7.75E-06 2E-03 1.63E-05 -1.41E-01
ETP-fw CTUe 5.78E+01 8E-02 2.9E-02 0 3.6E-02 1.89E-01 8E-03 -4.25E+00
HTP-c CTUh 3.67E-09 1.5E-12 1.52E-12 0 6.73E-13 1.61E-11 1.18E-12 1.37E-09
HTP-nc CTUh 1.25E-07 6.42E-11 6.7E-11 0 2.88E-11 1.59E-09 1.3E-10 1.65E-07
SQP SQP 4.68E+01 2.89E-04 1.6E-02 0 1.3E-04 1.49E-01 3E-03 -1.81E+00
PM = Potential incidence of disease due to PM emissions; IR = Potential Human exposure efficiency relative to U235; ETP-fw = Potential comparative
Toxic Unit for ecosystems; HTP-c = Potential comparative Toxic Unit for humans (cancerogenic); HTP-nc = Potential comparative Toxic Unit for humans
(not cancerogenic); SQP = Potential soil quality index
Disclaimer 1 – for the indicator “Potential Human exposure efficiency relative to U235”. This impact category deals mainly with the
eventual impact of low-dose ionizing radiation on human health of the nuclear fuel cycle. It does not consider effects due to possible
nuclear accidents, occupational exposure or radioactive waste disposal in underground facilities. Potential ionizing radiation from the
soil, radon and from some construction materials is also not measured by this indicator.
Disclaimer 2 – for the indicators “abiotic depletion potential for non-fossil resources”, “abiotic depletion potential for fossil resources”,
“water (user) deprivation potential, deprivation-weighted water consumption”, “potential comparative toxic unit for ecosystems”,
“potential comparative toxic unit for humans – cancerogenic”, “Potential comparative toxic unit for humans - not cancerogenic”,
“potential soil quality index”. The results of this environmental impact indicator shall be used with care as the uncertainties on these
results are high as there is limited experience with the indicator.
This EPD was created using a software tool.
References
EN 1300 Security Devices - High Security Locks for Secure
EN 1300:2019, Secure storage units - Storage Units - Requirements and Test Methods
Classification for high security locks according to their
resistance to unauthorized opening Further References
EN 15804 IBU 2021
EN 15804+A2:2019+AC:2021, General Instructions for the EPD programme of Institut Bauen
Sustainability of construction works — Environmental Product und Umwelt e.V. Version 2.0, Berlin: Institut Bauen und Umwelt
Declarations — Core rules for the product category of e.V., 2021. www.ibu-epd.com
construction products
GaBi
ECHA Sphera Solutions GmbH
European Chemical Agency Gabi Software System and Database for Life Cycle Engineering
19922020
ISO 14025 Version 10.0.0.71
DIN EN ISO 14025:201110, Environmental labels and University of Stuttgart
declarations — Type III environmental declarations — Leinfelden-Echterdingen
Principles and procedures
GaBi ts documentation
REACH GaBi life cycle inventory data documentation
Regulation (EC) No 1907/2006 of the European Parliament and (https://www.gabisoftware.com/support/gabi/gabidatabase-
of the Council on the Registration, Evaluation, Authorisation 2020-lcidocumentation/).
and Restriction of Chemicals (REACH)
LCA-tool dormakaba
RoHS Tool No.: BU-DOR-202105-LT1-EN.
2011/65/EU, Directive on the restriction of the use of certain Developed by Sphera Solutions GmbH
hazardous substances in electrical and electronic equipment
PCR Part A
UL 2058 PCR – Part A: Calculation Rules for the Life Cycle Assessment
UL 2058: 2005-06, Underwriters Laboratories, High- and Requirements on the Project Re-port according to EN
Security Electronic locks 15804+A2:2019, Version 1.0, 2020, Institut Bauen und Umwelt
e.V., www.ibu-epd.com.
VdS 2344
VdS 2344:2014-07, Procedure for the testing, approval PCR Part B
and certification of products and systems for fire PCR – Part B: Requirements on the EPD for Electronic and
protection and security technologies physical Access Control Systems, version 08/2021, Institut
Bauen und Umwelt e.V., www.ibu-epd.com.
VdS 2396
VdS 2396:2014-07, VdS Guidelines for Physical
5 Environmental Product Declaration - dormakaba - Safe Lock Auditcon
6 Environmental Product Declaration - dormakaba - Safe Lock Auditcon
Publisher
Institut Bauen und Umwelt e.V. +49 (0)30 3087748- 0
Hegelplatz 1 info@ibu-epd.com
10117 Berlin www.ibu-epd.com
Germany
Programme holder
Institut Bauen und Umwelt e.V. +49 (0)30 3087748- 0
Hegelplatz 1 info@ibu-epd.com
10117 Berlin www.ibu-epd.com
Germany
Author of the Life Cycle Assessment
dormakaba International Holding GmbH +49 2333 793-0
DORMA Platz 1 info.de@dormakaba.com
58256 Ennepetal www.dormakaba.com
Germany
Owner of the Declaration
dormakaba International Holding GmbH +49 2333 793-0
DORMA Platz 1 info.de@dormakaba.com
58256 Ennepetal www.dormakaba.com
Germany
7 Environmental Product Declaration - dormakaba - Safe Lock Auditcon
