ENVIRONMENTAL PRODUCT DECLARATION
as per ISO 14025 and EN 15804+A2
Owner of the Declaration Sonae Arauco, S.A.
Publisher Institut Bauen und Umwelt e.V. (IBU)
Programme holder Institut Bauen und Umwelt e.V. (IBU)
Declaration number EPD-SON-20230516-IBA2-EN
Issue date 10.01.2024
Valid to 09.01.2029
Particleboard, coated
Sonae Arauco, S.A.
www.ibu-epd.com | https://epd-online.com
1. General Information
Sonae Arauco, S.A. Particleboard, coated
Programme holder Owner of the declaration
IBU – Institut Bauen und Umwelt e.V. Sonae Arauco, S.A.
Hegelplatz 1 Calle Ulises 26­18
10117 Berlin 28043 Madrid
Germany Spain
Declaration number Declared product / declared unit
EPD­SON­20230516­IBA2­EN Particleboard, coated, per m2
This declaration is based on the product category rules: Scope:
Wood­based panels, 01.08.2021 This document refers toparticleboard, coated with melamine­impregnated
(PCR checked and approved by the SVR) paper, manufactured in the following plants of the Sonae Arauco group:
• Sonae Arauco Beeskow GmbH, Radinkendorfer Strasse 71,
15848 Beeskow, Germany
Issue date
• Sonae Arauco Deutschland GmbH ­ Nettgau Plant, Strohmweg
10.01.2024 1, 38489 Nettgau, Germany
• Sonae Arauco Portugal, SA, Estrada Nacional 17, nº 59 e 61,
3400­691 S.Paio de Gramaças (Oliveira do Hospital), Portugal
Valid to • Sonae Arauco South Africa (Pty) Ltd, Heidelberg Road, Rocky
Drift, White River, Republic of South Africa
09.01.2029
• Sonae Arauco España­ Soluciones de Madera, S.L., Carretera
Córdoba­Valencia Km 126, Estación Linares­Baeza, 23490
Linares (Jaén), Spain
The production volume of these plants covers 100 % of the total production
of particleboard by the Sonae Arauco group.
The owner of the declaration shall be liable for the underlying information
and evidence; the IBU shall not be liable with respect to manufacturer
information, life cycle assessment data and evidences.
The EPD was created according to the specifications of EN 15804+A2. In
the following, the standard will be simplified as EN 15804.
Dipl.­Ing. Hans Peters Verification
(Chairman of Institut Bauen und Umwelt e.V.)
The standard EN 15804 serves as the core PCR
Independent verification of the declaration and data according to ISO
14025:2011
internally X externally
Florian Pronold Mr Olivier Muller,
(Managing Director Institut Bauen und Umwelt e.V.) (Independent verifier)
1 Environmental Product Declaration ­ Sonae Arauco, S.A. ­ Particleboard, coated
2. Product
Name Value Unit
2.1 Product description/Product definition
Bending strength (longitudinal) according to
Coated particleboard is a panel­shaped wood­based material in 5.5 ­ 15 N/mm2
EN 310
accordance with EN 312 and EN 14322, which is manufactured
1050 ­
in a flat­pressing process by means of compression under heat E­module (longitudinal) according to EN 310 N/mm2
2050
of small wood particles with adhesive.
Due to their various densities and adhesive systems, coated Material dampness at delivery according to
5 ­ 13 %
particleboards can display a variety of material properties and EN 322
qualities like moisture resistance, fire­retardant or others. Tensile strength rectangular according to EN 0.14 ­
N/mm2
For the placing on the market of the product in the European 319 0.45
Union/European Free Trade Association (EU/EFTA) (with the Density limit deviation from average value
exception of Switzerland), Regulation (EU) No. 305/2011 (CPR) according to EN 323 +/­ 10 %
applies. When applicable, the product needs a declaration of
Strength tolerance according to EN 324 +/­ 0.3 mm
performance taking into consideration EN 13986:2004+A1:2015
Length and with tolerance according to EN
Wood-based panels for use in construction ­ Characteristics, +/­ 5.0 mm
324
evaluation of
conformity and marking and the CE marking. Edge straightness tolerance according to EN +/­ 1.5 mm/m
324
For the application and use the respective national provisions Perpendicularity according to EN 324 +/­ 2.0 mm/m
apply. Thickness swelling according to EN 317 12 ­ 17 %
2.2 Application Performance data of the product in accordance with the
The area of application for coated particleboard primarily declaration of performance with respect to its essential
involves decorative interior furnishings and furniture characteristics according to:
manufacturing. EN 312, Particleboards – Specifications
Particleboard can be classified into the following use classes EN 13986+A1, Wood-based panels for use in construction –
according to the requirements Characteristics, evaluation of conformity and marking.
established in EN 312:
Declaration of Performance (DoP)
• P1 General purpose boards for use in dry conditions
• P2 Boards for interior fitments (including furniture) for
For more details on technical information, please see the
use in dry conditions
respective products' Declaration of Performance (DoP)
• P3 Non load­bearing boards for use in humid conditions
available at:
• P4 Load­bearing boards for use in dry conditions
www.sonaearauco.com
• P5 Load­bearing boards for use in humid conditions
• P6 Heavy duty load­bearing boards for use in dry
Reference technical properties coated particle board according
conditions
to EN 14322:2021 are presented in the table below as
• P7 Heavy duty load­bearing boards for use in humid
reference values (special boards, as well as customized
conditions
products can have different values).
2.3 Technical Data
Due to the large variability of product properties and quality
grades, the table below only shows the range of technical
characteristics for classes P1 to P3 (boards for non­structural
applications).
Structural boards as well as customized products have different
technical characteristics from the ones shown.
2.4 Delivery status
Coated particleboard ranging in thicknesses from 6 to 40 mm
can be purchased as coated boards. The boards are offered in
standard formats. Custom formats are also available.
The following table includes typical dimension ranges for the
boards supplied worldwide. Some of the combinations for sizes
may not be available in all markets.
Thickness: 6 – 40
Width: 600 – 2650
Lenght: 800 – 5700
For updated information on available dimensions, please refer
to:
www.sonaearauco.com
2 Environmental Product Declaration ­ Sonae Arauco, S.A. ­ Particleboard, coated
2.5 Base materials/Ancillary materials This product contains substances listed in the ECHA candidate
Coated particleboard bonded with urea­ list (date: 08.06.2021) exceeding 0.1 percentage by mass: no
formaldehyde/melamine­urea­formaldehyde (UF/MUF) consist
of (dimensions as % by mass): This product contains other carcinogenic, mutagenic, reprotoxic
• Wood chips: approx. 85 % (CMR) substances in categories 1A or 1B which are not on the
• Water: 4 – 7% ECHA candidate list, exceeding 0.1 percentage by mass: no
• UF glue / MUF glue (urea resin, melamine urea resin): 8
– 10 % Biocide products were added to this construction product or it
• Paraffin wax emulsion: <1.5 % has been treated with biocide products (this then concerns a
• Impregnated paper: 0.5 – 3 % treated product as defined by the (EU) Ordinance on Biocide
Coated particleboard bonded with polymeric diphenylmethane Products No. 528/2012: no
diiscocyanate (PMDI) consist of (dimensions as % by mass):
2.6 Manufacture
• Wood chips: approx. 85 % The wood is chipped, screened and dried. Surface layer and
• Water: 4 – 7 % core layer materials are then glued and scattered on a forming
• PMDI glue: 8 – 10 % belt as a particles' mat. This is pressed into panels under high
• Paraffin wax emulsion: < 1.5 % pressure in a hot press. The panels are trimmed, picked and
• Impregnated paper: 0.5 – 3 % sanded on both sides after cooling.
Wood from indigenous, largely regional forest plantations is Finally, the panels are coated with melamine­impregnated
used for manufacturing particleboard. This wood is typically paper in a short­cycle press.
procured from forests an average radius of 250 km of the
plants' locations. All leftovers incurred during board manufacture are redirected
into the process or used as fuel to supply the energy needs of
Furthermore, sawmill residues and recycled wood are also the manufacturing process on site.
used as key raw materials in the production of particleboard.
A process diagram is presented below.
The entire range can be made available on request as FSC®
certified or PEFC (program for the endorsement of forest
certification) certified products.
Additionally, the complete range includes CE­marked products.
regulatory guidelines are required. The reference occupational
exposure limit values are complied with.
The production sites are certified according to the following
standards: Emissions into air: Waste air generated during production is
cleaned in accordance with regulatory requirements. Emissions
• ISO 9001
have to comply with the values specified by the operation
• ISO 45001
licenses of the different sites, specified according to national
• ISO 50001 (European sites).
laws.
2.7 Environment and health during manufacturing
Health protection: Due to the manufacturing conditions, no Emissions into water/soil: No normal process contamination
special health protection measures over and beyond the of water or soil exists. Typically, the
production process of coated particleboard does not have any
3 Environmental Product Declaration ­ Sonae Arauco, S.A. ­ Particleboard, coated
production­related waste water.
Noise: Noise surveys are required and are performed for each 2.13 Extraordinary effects
site according to respective national regulations. Noise­ Fire
intensive plant areas such as chipping are encapsulated or Fire retardant classification of coated particleboard is done
protected appropriately by structural measures. Whenever according to EN 13986. Fire retardant classes are defined in
necessary (close to non­encapsulated areas), the use of ear accordance with EN 13501-1.
protection is required (PPE, Personal Protective Equipment) Fire protection
within Sonae Arauco sites, as an additional safety measure.
Name Value
The production sites are all ISO 14001 certified.
Building material class D
2.8 Product processing/Installation Smoke gas development S2
Sonae Arauco coated particleboard can be sawn, milled and Burning droplets d0
drilled using standard machinery or (electric) power tools.
Surfaced particleboard with improved fire reaction is available
Carbide­tipped tools should be given preference, especially on
with, classification B­s2,d0
circular saws.
Respiratory protection should be worn when using hand­held
equipment without suction devices.
Water
Please refer to the respective devices' datasheets for further
No ingredients are washed out which could be hazardous to
processing recommendations.
water. Particleboards are not resistant to permanent exposure
2.9 Packaging to water.
Sonae Arauco coated particleboards are supplied on squared
timber bound by plastic or metal bands and covered with Mechanical destruction
corrugated cardboard and, on the bottom, with a cover board. Mechanical destruction of coated particleboards can result in
Particleboard and steel or PET packing bands for transport sharp edges on the broken panel edges (risk of injury).
packaging can be sorted and directed to the recycling circuits. If
2.14 Re-use phase
re­use or recycling is impractical, the packaging should not be
Recycling: Sonae Arauco coated particleboards from
landfilled, but rather directed towards energy recovery.
construction can be collected separately and utilised in the
Packaging disposal information is available at:
manufacture of particleboard. This is based on the condition
www.sonaearauco.com
that the wooden boards are not fully glued.
2.10 Condition of use
The components making up coated particleboard correspond Energy recovery: Due to the high heating value of approx.
with the base material compositions as outlined in Clause 2.6. 16.6 MJ/kg at 20 % moisture content assumed for post­
During hot pressing, the binding agent is linked irreversibly by consumer boards, coated particleboards can be used for
means of poly­condensation and firmly bonded with the wood. energy recovery and the generation of heat and electricity (e.g.
The binding agents are chemically and stably bound to the in CHP plants), following the cascading principle for wood.
wood.
2.15 Disposal
VOC emissions: Sonae Arauco coated particleboards are
Sonae Arauco coated particleboard leftovers and residual
labelled as class A+ according to the French regulation on the
materials incurred as a result of demolition measures on the
labelling of emissions of volatile pollutants from construction
building sites should be primarily directed towards material
and decoration products (with reference to the wall scenario, as
recycling. If this is not possible, they must be directed toward
a worst case).
energy recovery instead of landfilling.
Sonae Arauco particleboard coated with melamine impregnated
Waste code according to the European List of Waste: 17 02 01
paper at an average area weight of 11.1 kg/m2 stores 16.5 kg
CO 2/m2 equivalent over its service life. 2.16 Further information
Further information such as technical datasheets, etc. can be
2.11 Environment and health during use
downloaded under:
Environmental protection: According to current information,
water, air and soil are not exposed to any dangers when the www.sonaearauco.com
respective products outlined above are used as designated.
Health protection: According to current information, no
damage to or impairment of health can be anticipated when
particleboards are used as designated. With the exception of
low volumes of formaldehyde for UF/MUF­bonded
particleboard, VOC emissions from products are negligible, and
are natural wood ingredients.
2.12 Reference service life
Due to the wide range of applications of Sonae Arauco coated
particleboard, no reference service life is declared.
4 Environmental Product Declaration ­ Sonae Arauco, S.A. ­ Particleboard, coated
3. LCA: Calculation rules
leaving the production system in the modules A5 and C3.
3.1 Declared Unit Therefore, module D covers the avoided burdens from recycling
The declared unit for the LCA is 1 m2 of average Sonae Arauco and from energy recovered from the waste treatment in module
particleboard. A5 as well as the transport of the obsolete boards to a biomass
combustion plant, the combustion process itself and the loads
Information on the declared unit
and benefits of the substitution of fossil fuels and/or electricity.
Name Value Unit
Substitution effects in module D are always calculated for the
Declared unit 1 m2 net amount of secondary material or secondary fuel of the
Grammage 11.1 kg/m2 product system in line with EN 16485.
Layer thickness 0.0165 m
3.3 Estimates and assumptions
The weighted average was calculated based on production For the quantification of the net flows of recycled wood (input of
volumes from the plants in all countries where Sonae Arauco post­consumer wood used as a fuel minus post­consumer
was operating in 2021 (some plants 2020). wood exiting the product system into module D for energy
recovery), it was assumed that all inputs of post­consumer
3.2 System boundary
wood are used as a fuel; inputs of post­consumer wood beyond
Type of the EPD: cradle­to­gate with modules C1 to C4 and the need of wood fuel used in production was considered to be
module D (A1­A3, C and D) used as a recycled material input. Beyond that, no relevant
estimates or assumptions had to be made beyond the
Modules A1 – A3 of the production stage cover the information provided in this EPD.
manufacturing of the products, including raw material extraction
and processing, energy generation, the production of ancillary 3.4 Cut-off criteria
products and packaging materials, transport, as well as all All data were taken into account that resulted from the data
waste treatment processes. Eventual benefits of recycling or collection procedure in the plants, e.g. related to fuels, raw
energy recovery are neglected. material input, use of ancillary materials, waste flows,
emissions into the air, water use, waste water, transport means
The resource aspects of wood were inventoried via material and transport distances, etc..
inherent properties such as resource extraction of CO from the Expenses for the general management, research &
2
atmosphere and the lower heating value as the use of development, administration and marketing – if known – were
renewable energy. Material inherent properties are subject to not taken into account.
co­product allocation as ruled in EN 15804.
The production of eventual packaging of ancillary material or
Module A4 covers the transport of the product from the other inputs used during production (and some of the reported
production site to the construction site by a lorry over a default wastes) were generally neglected; in most cases reusable bins
distance of 460 km. or containers are used. In addition, the amounts of reported
(unspecific) wastes are so small that their production can be
Module A5 covers the transport of the packaging material from considered not relevant for the life cycle assessment. Additional
the construction site and its disposal. Default end­of­waste plant specific information can be found in the respective
states for the packaging materials from the packed products at chapters for each plant.
the construction site are defined in analogy for wastes
occurring in modules A1­A3. Eventual further inputs for the Beyond that some plants reported ancillary materials that were
installation of the products are not considered due to the broad cut off due to very small amounts and as inputs not directly
applicability of the assessed products. related to production processes but to the maintenance of
The substituted primary material from the net amount of infrastructure, e.g. acetylene and oxygen for soldering, etc.
recycled material and from recovered energy exported from the With this approach mass and energy flows below 1 percent of
product system in Module A5 is declared in Module D. total mass and energy flows caused by the declared products
were included in the assessment.
Module C1 manual deconstruction isassumed. The declared
values are thus 0. Beyond that, no material or energy flows were neglected that
would have been known by the persons responsible for the
Module C2 includes the transport of the de­constructed product project and that could have been expected to contribute
to a recycling centre by over 50 km. significantly to the environmental indicators declared. It can
thus be assumed that the total contribution of the neglected
Module C3 covers the preparation of the post­consumer board processes is not higher than 5 % of the declared impact
to become a secondary fuel; the end­of­waste status for categories.
recycled wood­based boards is defined as the point where they
3.5 Background data
have been sorted and chipped, ready to be used as secondary
fuels. Datasets from ecoinvent 3.8 were used as background data
In line with EN 16485, the export of the biogenic carbon stored exclusively. Therefore, the latest update of the background data
in the board, expressed in CO ­equivalent is also reported in took place in 2021.
2
module C3. 3.6 Data quality
The requirements on the data quality and the background data
Module C4 is not relevant for the assumed end­of­life scenario.
correspond to the
The declared values are thus 0.
provisions in EN 15804:
Module D compiles all the benefits and burdens associated with • Data are as current as possible. Datasets used for
the secondary fuels, secondary materials and exported energy calculations were updated within the last 10 years for
5 Environmental Product Declaration ­ Sonae Arauco, S.A. ­ Particleboard, coated
generic data and within the last 5 years for producer­ implying that the content of primary energy in products and
specific data; packaging is allocated as the main inputs/outputs of a unit
• Datasets are based on 1­year averaged data as a process.
general rule; In the case of sites where several products were produced and
• The time period over which inputs to and outputs from no product­specific information was available, all inputs and
the system are accounted for is 100 years from the year outputs related to production processes were attributed based
for which the data set is deemed representative; on a total mass of production; packaging material was
• The technological coverage reflects the physical reality attributed based on a total volume of the production. Inputs and
of the declared products; outputs for coating processes that could not be separated from
• The background datasets comply with the quality the data on plant level were conservatively attributed to the
guidelines of ecoinvent v.3; deviations from the particleboard production.
methodological prescriptions of EN 15804 cannot be Post­consumer secondary wood is used as an input to produce
excluded but are considered not significant in the particleboard; for this input as well as for the end­of­life
context of this EPD. scenario, the end­of­waste status was defined after the sorting
and chipping of the wood­based board in line with EN 16485
3.7 Period under review (see also clause 3.2). In analogy, particleboard leaving the
The company data gathered for this EPD represents the year product system at the end­of­life is considered a secondary
2021 (for some plants 2020). fuel; its combustion and the benefits of energy recovery are
declared in module D.
3.8 Geographic Representativeness
Waste packaging in module A5 was considered not to reach the
Land or region, in which the declared product system is end­of­waste state as a fuel. Its incineration is reported in A5,
manufactured, used or handled at the end of the product´s the benefits of energy recovery in module D. The benefits of the
lifespan: Europe recycling of minor amounts of packaging materials are
disregarded.
No co­product allocation was made in the modelling of the
3.9 Allocation
foreground data of the life cycle assessment underlying this
The inventories for the wood inputs were taken from ecoinvent
EPD.
v.8. In ecoinvent, the forestry processes are modelled on a
mass­basis and sawmilling processes are allocated based on 3.10 Comparability
revenues of the different co­products of a joint co­production
Basically, a comparison or an evaluation of EPD data is only
process.
possible if all the data sets to be compared were created
Waste generated by edge­trimming and cut­size saws is used
according to EN 15804 and the building context, respectively
internally for energy generation. Some plants sell minor
the product­specific characteristics of performance, are taken
quantities of bark, waste wood or electricity from co­generation.
into account.
No impacts are allocated to these outputs.
Datasets from ecoinvent v3.8 were used as background data
Biogenic carbon (content) is modelled manually thus reflects
exclusively.
the real physical flows; this is not the case for primary energy,
4. LCA: Scenarios and additional technical information
electricity (according to specifications of MWI plants in
Characteristic product properties of biogenic carbon ecoinvent 3.8).
Note: 1 kg of biogenic carbon is equivalent to 44/12 kg of CO .
2
Deconstruction(C1)
Information on describing the biogenic carbon content at
Manualdeconstruction is assumed. The declared values are
factory gate
thus 0.
Name Value Unit
Biogenic carbon content in product 4,50 kg C Transport to waste treatment (C2)
Biogenic carbon in packaging 0,0540 kg C This module includes the transport of the de­constructed
product to a recycling centre by a lorry (15 % emissions class
EURO 5; 85 % emissions class EURO 6) by over 50 km.
The following technical information is a basis for the declared
modules or can be used for developing specific scenarios in the
Waste treatment (C3)
context of a building assessment if modules are not declared
12.1 kg of coated particleboard are chipped and exported from
(MND).
the product life cycle into module D, assuming a moisture
content of 20 % and a lower heating value of 16,2 MJ/kg.
Transport to the construction site (A4)
The biogenic carbon stored in the product and the content of
The product is transported from the production site to the
primary energy are exported from the product system as
construction site by a lorry (15 % emissions class EURO 5; 85
material inherent properties.
% emissions class EURO 6) over a default distance of 460 km.
Disposal (C4)
Installation into the building (A5)
This module is not relevant for the assumed end­of­life
Eventual further inputs for the installation of the products are
scenario. The declared values are thus 0.
not considered due to the broad applicability of the assessed
products.
Reuse, recycling, recovery potential (D)
An average transport distance of 30 km was assumed for
According to default assumptions in other IBU EPDs, post­
packaging waste from the construction site to the recycling
consumer wood is used as a secondary fuel for energy
plant or to the municipal waste incineration plant. The municipal
recovery in a biomass combustion plant with an overall energy
waste incineration plant is assumed to have an overall energy
efficiency of 93 % related to the lower heating value of the fuel
efficiency of 53 % related to the lower heating value of the
input; 91 % of the recovered energy is heat, 9 % is electricity.
waste input; 92 % of the recovered energy is heat, 8 % is
6 Environmental Product Declaration ­ Sonae Arauco, S.A. ­ Particleboard, coated
5. LCA: Results
DESCRIPTION OF THE SYSTEM BOUNDARY (X = INCLUDED IN LCA; MND = MODULE OR INDICATOR NOT DECLARED; MNR
= MODULE NOT RELEVANT)
Benefits and
Construction loads beyond
Product stage Use stage End of life stage
process stage the system
boundaries
la ire ta m w a Ry lp p u s tro p s n a rT g n iru tc a fu n a M e h t m o rf tro p s n a rTe tis e h t o t e ta g y lb m e s s A e s U e c n a n e tn ia M ria p e R tn e m e c a lp e R tn e m h s ib ru fe R y g re n e la n o ita re p Oe s u re ta w la n o ita re p Oe s u n o itc u rts n o c ­e Dn o itilo m e d tro p s n a rT g n is s e c o rp e ts a W la s o p s iD ­e s u e R­y re v o c e R­g n ilc y c e Rla itn e to p
A1 A2 A3 A4 A5 B1 B2 B3 B4 B5 B6 B7 C1 C2 C3 C4 D
X X X X X MND MND MNR MNR MNR MND MND X X X X X
RESULTS OF THE LCA - ENVIRONMENTAL IMPACT according to EN 15804+A2: Particleboard, coated with melamine-
impregnated paper, per m²
Parameter Unit A1-A3 A4 A5 C1 C2 C3 C4 D
GWP­total kg CO 2 eq ­9.11E+00 8.43E­01 2.11E­01 0 1.18E­01 1.66E+01 0 ­5.17E+00
GWP­fossil kg CO 2 eq 7.57E+00 8.43E­01 1.26E­02 0 1.18E­01 9.83E­02 0 ­5.17E+00
GWP­biogenic kg CO 2 eq ­1.67E+01 0 1.98E­01 0 0 1.65E+01 0 0
GWP­luluc kg CO 2 eq 1.16E­02 3.36E­04 7.4E­07 0 5.6E­05 2.25E­04 0 ­3.22E­03
ODP kg CFC11 eq 1.08E­06 1.95E­07 1.05E­09 0 2.67E­08 4.93E­09 0 ­1.18E­06
AP mol H+ eq 4.72E­02 2.55E­03 6.04E­05 0 3.56E­04 5.24E­04 0 ­9.14E­03
EP­freshwater kg P eq 2.86E­04 5.99E­06 2.55E­08 0 9.67E­07 1.02E­05 0 ­1.43E­04
EP­marine kg N eq 8.12E­03 5.59E­04 2.72E­05 0 7.46E­05 7.12E­05 0 ­9.59E­04
EP­terrestrial mol N eq 1.1E­01 6.21E­03 3.07E­04 0 8.31E­04 8.14E­04 0 ­1.08E­02
kg NMVOC
POCP 3.02E­02 2.25E­03 9.1E­05 0 3.02E­04 2.29E­04 0 ­4.71E­03
eq
ADPE kg Sb eq 8.93E­05 2.98E­06 7.4E­09 0 5.42E­07 2.7E­07 0 ­3.27E­06
ADPF MJ 1.49E+02 1.28E+01 6.73E­02 0 1.77E+00 2.05E+00 0 ­1.55E+02
m3 world eq
WDP 8.27E+00 3.88E­02 3.58E­04 0 5.88E­03 2.38E­02 0 ­1.41E­01
deprived
GWP = Global warming potential; ODP = Depletion potential of the stratospheric ozone layer; AP = Acidification potential of land and water; EP =
Eutrophication potential; POCP = Formation potential of tropospheric ozone photochemical oxidants; ADPE = Abiotic depletion potential for non­fossil
resources; ADPF = Abiotic depletion potential for fossil resources; WDP = Water (user) deprivation potential)
RESULTS OF THE LCA - INDICATORS TO DESCRIBE RESOURCE USE according to EN 15804+A2: Particleboard, coated with
melamine-impregnated paper, per m²
Parameter Unit A1-A3 A4 A5 C1 C2 C3 C4 D
PERE MJ ­9.99E+01 1.79E­01 2.14E+00 0 2.95E­02 3.56E­01 0 ­5.13E+00
PERM MJ 1.73E+02 0 ­2.14E+00 0 0 ­1.71E+02 0 0
PERT MJ 7.32E+01 1.79E­01 7.64E­04 0 2.95E­02 ­1.71E+02 0 ­5.13E+00
PENRE MJ 1.22E+02 1.28E+01 1.73E­01 0 1.77E+00 2.07E+00 0 ­1.54E+02
PENRM MJ 2.73E+01 0 ­1.06E­01 0 0 ­2.72E+01 0 0
PENRT MJ 1.49E+02 1.28E+01 6.73E­02 0 1.77E+00 ­2.51E+01 0 ­1.54E+02
SM kg 2.69E+00 0 0 0 0 0 0 0
RSF MJ 6.92E+01 0 0 0 0 0 0 1.05E+02
NRSF MJ 0 0 0 0 0 0 0 3.37E+01
FW m3 2.15E­01 1.35E­03 5.67E­05 0 5.67E­05 1.25E­03 0 ­1.18E­02
PERE = Use of renewable primary energy excluding renewable primary energy resources used as raw materials; PERM = Use of renewable primary
energy resources used as raw materials; PERT = Total use of renewable primary energy resources; PENRE = Use of non­renewable primary energy
excluding non­renewable primary energy resources used as raw materials; PENRM = Use of non­renewable primary energy resources used as raw
materials; PENRT = Total use of non­renewable primary energy resources; SM = Use of secondary material; RSF = Use of renewable secondary fuels;
NRSF = Use of non­renewable secondary fuels; FW = Use of net fresh water
RESULTS OF THE LCA – WASTE CATEGORIES AND OUTPUT FLOWS according to EN 15804+A2:
Particleboard, coated with melamine-impregnated paper, per m²
Parameter Unit A1-A3 A4 A5 C1 C2 C3 C4 D
HWD kg 2.07E­04 3.33E­05 5.34E­08 0 4.75E­06 9.52E­07 0 ­1.67E­04
NHWD kg 1.57E+00 6.71E­01 1.67E­03 0 7.59E­02 1.36E­02 0 1.86E­01
RWD kg 6.6E­04 1.85E­04 9.09E­07 0 2.54E­05 2.68E­05 0 ­4.82E­04
CRU kg 0 0 0 0 0 0 0 0
MFR kg 1.29E­02 0 5.59E­03 0 0 0 0 0
MER kg 0 0 0 0 0 1.21E+01 0 0
EEE MJ 4.48E­04 0 7.63E­02 0 0 0 0 0
EET MJ 5.15E­03 0 8.77E­01 0 0 0 0 0
7 Environmental Product Declaration ­ Sonae Arauco, S.A. ­ Particleboard, coated
HWD = Hazardous waste disposed; NHWD = Non­hazardous waste disposed; RWD = Radioactive waste disposed; CRU = Components for re­use;
MFR = Materials for recycling; MER = Materials for energy recovery; EEE = Exported electrical energy; EET = Exported thermal energy
RESULTS OF THE LCA – additional impact categories according to EN 15804+A2-optional:
Particleboard, coated with melamine-impregnated paper, per m²
Parameter Unit A1-A3 A4 A5 C1 C2 C3 C4 D
Disease
PM 3.82E­07 5.4E­08 8.48E­10 0 6.52E­09 1.6E­09 0 ­7.12E­09
incidence
IR kBq U235 eq 3.02E­01 5.55E­02 2.67E­04 0 7.71E­03 1.81E­02 0 ­2.79E­01
ETP­fw CTUe 1.76E+02 1E+01 5.54E­02 0 1.45E+00 1.16E+00 0 ­9.58E+00
HTP­c CTUh 4.99E­08 3.22E­10 3.28E­11 0 5.23E­11 5.51E­11 0 1.28E­09
HTP­nc CTUh 1.3E­07 1.02E­08 1.22E­10 0 1.41E­09 9.99E­10 0 2.5E­09
SQP SQP 3.78E+02 8.88E+00 1.34E­02 0 1.05E+00 3.16E­01 0 ­4.05E+00
PM = Potential incidence of disease due to PM emissions; IR = Potential Human exposure efficiency relative to U235; ETP­fw = Potential comparative
Toxic Unit for ecosystems; HTP­c = Potential comparative Toxic Unit for humans (cancerogenic); HTP­nc = Potential comparative Toxic Unit for humans
(not cancerogenic); SQP = Potential soil quality index
Disclaimer 1 – for the indicator “Potential Human exposure efficiency relative to U235”. This impact category deals mainly with the
eventual impact of low­dose ionizing radiation on human health of the nuclear fuel cycle. It does not consider effects due to possible
nuclear accidents, occupational exposure or radioactive waste disposal in underground facilities. Potential ionizing radiation from the
soil, radon and from some construction materials is also not measured by this indicator.
Disclaimer 2 – for the indicators “abiotic depletion potential for non­fossil resources”, “abiotic depletion potential for fossil resources”,
“water (user) deprivation potential, deprivation­weighted water consumption”, “potential comparative toxic unit for ecosystems”,
“potential comparative toxic unit for humans – cancerogenic”, “Potential comparative toxic unit for humans ­ not cancerogenic”,
“potential soil quality index”. The results of this environmental impact indicator shall be used with care as the uncertainties on these
results are high as there is limited experience with the indicator.
6. LCA: Interpretation
Figure 1 illustrates the contribution of each life cycle stage to from module A1­C4 = 100 %) for coated particleboard.
the overall indicator results of the impact assessment (impact
construction site whereas the contributions from other modules
Figure 1: Environmental impacts of particleboard coated of the life cycle are negligible.
with melamine-impregnated paper along its life cycle Loads and benefits beyond the life cycle (module D) are
(impacts from production modules A1-C4 = 100 %) negative (benefits > loads) whereas major contributions occur
for the ODP, the GWP­fossil and for the ADPF; these benefits
Figure 1 illustrates that the environmental profile of coated basically stem from the use of the particleboard as secondary
particleboard is dominated by the production phase (modules fuel and its related substitution of natural gas and electricity
A1­A3). Minor contributions stem from transport to the from the grid from the recovered energy.
8 Environmental Product Declaration ­ Sonae Arauco, S.A. ­ Particleboard, coated
Figure 2 illustrates that the biogenic carbon stored in the
particleboard coated with melamine im­pregnated paper,
expressed as CO ­equivalent, is higher than the CO
2 2
emissions from fossil sources, leading to a negative GWP for
the production module A1­A3. The potential substitution effect
in mod­ule D offsets the GHG emissions during the production
phase (module A1­A3).
Figure 2: Greenhouse Gas balance of particleboard coated
with melamine-impregnated paper
The GWP is dominated by CO emissions and removals.
2
7. Requisite evidence
7.1 Formaldehyde Cologne, Germany
Test reports, date: Report 0001122970/20 AZ 581067,
For UF/MUF bonded boards: 20.09.2022
(tests made on raw boards) Result: The limit values are complied with. Limits evaluated
according to the Toy safety-directive 2009/48/EC: category 3:
Measuring agency: MPA Eberswalde materialprüfanstalt Scraped of toy material.
Brandenbutg GmbH ­ Holz uns Holzschutz
Test report, date: No 31/23/4155/01/QT issued at 02.04.2023 Metal analysis for Iberian market, based on quarterly analysis:
Result: ZE05 ­ Certification of wood­based panels regarding Measuring agency: IDIT, Instituto de Desenvolvimento e
formaldehyde emissions in accordance with the German Inovação Tecnológica, Portugal
Chemicals Prohibition Ordinance (ChemVerbotsV) and based Test reports, date: 2057/2015 & 2058/2015, 22 December
on DIBt Guideline 100. Test procedure according to EN 717-1. 2015
Calculated formaldehyde concentration was 0,054 ppm Result: The limit values outlined in the EPF voluntary
according to ChemVerbotsV (concentration of EN 717­1 standards on the use of recycled wood are complied with. Limit
multiplied by factor 2), compying with the limit 0,1ppm. values in mg/kg: As 25, Pb 90, Cd 50, Cr 25, Cu 40, Hg 25, Cl
1000, F 100, PCP 5 and Creosote 0.5. .
Measuring agency: MPA Eberswalde materialprüfanstalt
Brandenbutg GmbH ­ Holz uns Holzschutz 7.3 TVOC emissions
Test report, date: No. 31/23/3768/01/QT issued on the
25.01.2023 Measuring agency: Eurofins Denmark
Result: ZE05 ­ Certification of wood­based panels regarding Test report, date: 392­2002­00522601­B­EN, issued on the
formaldehyde emissions in accordance with the German 05.01.2023
Chemicals Prohibition Ordinance (ChemVerbotsV) and based Result: Classification A+ according to French regulation
on DIBt Guideline 100. Test procedure according to EN 717-1. Decrée of March 2011 (DEVL1101903D) and Arrêté of April
Calculated formaldehyde concentration was 0,045 ppm 2011 (DEVL1104875A) modified in February 2012
according to ChemVerbotsV (concentration of EN 717-1 (DEVL1133129A)
multiplied by factor 2), compying with the limit 0,1ppm Compliant with ABG/AgBB (Ausschuss zur gesundheitlichen
Bewertung von Bauprodukten (June 2021).
Measuring agency: Fraunhofer Institute for Wood Research
Wilhelm­Klauditz­Institut WKI
Test report, date: No. QA­2021­0453 issued on the
AgBB overview of results (28 days)
04.03.2021
Name Value Unit
Results: Determination of the formaldehyde release according
to JIS A1460. An average value of 0,1 mg/litre was determined TVOC (C6 ­ C16) 80 μg/m3
with individual values of 0,06 mg/litre and 0,09 mg/litre Sum SVOC (C16 ­ C22) < 5 μg/m3
corresponding to the F4Stars level.
R (dimensionless) 0.11 ­
7.2 Checking for the pretreatment of the substances used
VOC without NIK < 5 μg/m3
(tests made on raw boards) Carcinogenic Substances < 1 μg/m3
Measuring agency: TÜV Rheinland LGA Products GmbH,
9 Environmental Product Declaration ­ Sonae Arauco, S.A. ­ Particleboard, coated
7.4 PCP/Lindane
AgBB overview of results (3 days [µg/m³])
(tests made on raw boards)
Name Value Unit
Measuring agency: EPH Entwicklungs­ und Prüflabor
TVOC (C6 ­ C16) 20 μg/m3 Holztechnologie GmbH, Zellescher Weg 24, D­01217 Dresden
Sum SVOC (C16 ­ C22) < 5 μg/m3 Test reports, date: Standard product Supervision Report 02­
2015, Order 2515024/3­2, dated 18 December 2015. P3
R (dimensionless) 0.15 ­
product Supervision Report 02­2015, Order 2515024/3­1, dated
VOC without NIK < 5 μg/m3
18 December 2015
Carcinogenic Substances < 1 μg/m3 Result: The wood preservative agents pentachlorophenol
(PCP) and lindane could not be determined in the sample of
boards examined, or fulfilled the limit value of 5 mg/kg.
Limit of determination: 0.05 mg/kg.
8. References
Product category rules of IBU chamber method.
IBU (2021) EN 12524
IBU (2021): General Instructions for the EPD Programme of the EN 12524:2000, Building materials and products –
Institut Bauen und Umwelt e.V. (General Instructions for the Hygrothermal properties – Tabulated design values.
IBU EPD Programme). Version 2.0, Institut Bauen und Umwelt,
Berlin. EN 13501
EN 13501­1:2019, Fire classification of construction products
IBU (2021) and building elements – Classification using test data from
IBU (2021): PCR Part A: Calculation rules for the life cycle reaction to fire tests.
assessment and requirements for the project report according
to EN 15804+A2:2019. Version 1.3., Institut Bauen und Umwelt, EN 13986
Berlin. EN 13986:2015, Wood­based panels for use in construction –
Characteristics, evaluation of conformity and marking.
IBU (2023)
IBU (2023): PCR Part B: Requirements on the EPD for wood­ EN 14322
based panels. Version 2023/04, Institut Bauen und Umwelt, EN 14322:2021, Wood­based panels – Melamine faced boards
Berlin. for interior uses – Definitions, requirements and classification.
EN 15804
Standards and legal documents EN 15804+A2:2019 + AC:2021, Sustainability of construction
works – Environmentalproduct declarations – Core rules for the
EN 310 product category construction products.
EN 310:1993, Wood­based panels – Determination of modulus
of elasticity in bending and of bending strength. EN 16485
EN 16485:14­07, Round and sawn timber – Environmental
EN 312 Product Declarations –
EN 312:2010, Particleboards – Specifications. Product category rules for wood and wood­based products for
use in construction.
EN 317
EN 317:1993, Particleboards and Fibreboards – Determination ISO 9001
of swelling in thickness after immersion in water. ISO 9001:2015, Quality management systems – Requirements.
EN 319 ISO 14001
EN 319:1993, Particleboards and fibreboards – Determination ISO 14001:2015, Environmental management systems –
of tensile strength perpendicular to the plane of the board. Requirements with guidance for use.
EN 322 ISO 14025
EN 322:1993, Wood­based panels – Determination of moisture ISO 14025:2006­07, Environmental labels and declarations ­
content. Type III Environmental declarations ­ Principles and
procedures.
EN 323
EN 323:1993, Wood­based panels – Determination of density. ISO 14044
EN ISO 14044:2006­07, Environmental management ­ Life
EN 324 cycle assessment ­ Requirements and guidance (ISO
EN 324­1:1993, Wood­based panels – Determination of 14044:2006); German and English versions EN ISO
dimensions of boards – Determination of thickness, width and 14044:2006.
length.
EN 324­2:1993, Wood­based panels – Determination of ISO 45001
dimensions of boards – Determination of squareness and edge DIN ISO 45001:2018­06, Occupational health and safety
straightness. management systems – Requirements with guidance for use.
EN 717-1 ISO 50001
EN 717­1:2005­01, Wood­based panels – Determination of ISO 50001:2018, Energy management systems –
formaldehyde release – Formaldehyde emission by the Requirements with guidance for use.
10 Environmental Product Declaration ­ Sonae Arauco, S.A. ­ Particleboard, coated
Council of 18 June 2009 on the safety of toys (Text with EEA
ISO 16000 relevance).
ISO 16000­11:2006, Indoor air – Part 11: Determination of the
emission of volatile organic compounds from building products COUNCIL REGULATION (EU) No 333/2011
and furnishing – Sampling, storage of samples and preparation COUNCIL REGULATION (EU) No 333/2011 of 31 March 2011
of test specimens. establishing criteria determining when certain types of scrap
metal cease to be waste under Directive 2008/98/EC of the
JIS A 1460 European Parliament and of the Council.
JIS A 1460:2015: Determination of the emissions of
formaldehyde from building boards – Desiccator method. Regulation on the European Waste List (Waste index)
http://www.gesetze­im­internet.de/avv/anlage.html
ECHA-List
The Candidate List of substances of very high concern, ChemVerbotsV,
available via Chemikalien­Verbotsverordnung (German Regulation on the
https://echa.europa.eu/nl/­/four­newsubstances­added­to­the­ Prohibition of Chemicals, from 14 October 1993).
candidate­list.
Additional references
Regulation on biocidal products
REGULATION (EU) No 528/2012 OF THE EUROPEAN BBSR 2017
PARLIAMENT AND OF THE COUNCIL of 22 May 2012 Bundesinstitut für Bau­, Stadt­ und Raumforschung Service Life
concerning the making available on the market and use of of Building Components; version 24.02.2017.
biocidal products.
https://www.nachhaltigesbauen.de/fileadmin/pdf/Nutzungsdauer_Bauteile/BNB_Nutzungsdauern_von_Bauteilen_2017­
Regulation (EU) Nr. 305/2011(CPR) 2­24.pdf
REGULATION (EU) No 305/2011 OF THE EUROPEAN
PARLIAMENT AND OF THE COUNCIL of 9 March 2011 laying DIBt Guideline 100
down harmonised conditions for the marketing of construction Regulation on the classification and external supervision of
products and wood­based panels regarding formaldehyde emission (DIBt ­
repealing Council Directive 89/106/EEC. Guideline 100), dated June 1994
Toy safety-directive 2009/48/EC ecoinvent v3.8
Directive 2009/48/EC of the European Parliament and of the Life cycle database ecoinvent v3.8, 12/2021. ecoinvent, Zürich.
11 Environmental Product Declaration ­ Sonae Arauco, S.A. ­ Particleboard, coated
Publisher
Institut Bauen und Umwelt e.V. +49 (0)30 3087748­ 0
Hegelplatz 1 info@ibu­epd.com
10117 Berlin www.ibu­epd.com
Germany
Programme holder
Institut Bauen und Umwelt e.V. +49 (0)30 3087748­ 0
Hegelplatz 1 info@ibu­epd.com
10117 Berlin www.ibu­epd.com
Germany
Author of the Life Cycle Assessment
Dr. Frank Werner ­ Umwelt & Entwicklung + 41 (0)44 241 39 06
Kammelenbergstrasse 30 frank@frankwerner.ch
9011 St. Gallen http://www.frankwerner.ch/
Switzerland
Owner of the Declaration
Sonae Arauco, S.A. (+34) 918 070 701
Calle Ulises 26­18 products@sonaearauco.com
28043 Madrid www.sonaearauco.com
Spain
12 Environmental Product Declaration ­ Sonae Arauco, S.A. ­ Particleboard, coated
