ENVIRONMENTAL-PRODUCT DECLARATION
as per ISO 14025 and EN 15804+A1
Owner of the Declaration dormakaba International Holding GmbH
Publisher Institut Bauen und Umwelt e.V. (IBU)
Programme holder Institut Bauen und Umwelt e.V. (IBU)
Declaration number EPD-DOR-20210083-IBI1-EN
Issue date 28/06/2021
Valid to 27/06/2026
ST PRO Green RC
dormakaba Deutschland GmbH
www.ibu-epd.com | https://epd-online.com
1. General Information
dormakaba Deutschland GmbH ST PRO Green RC
Programme holder Owner of the declaration
IBU – Institut Bauen und Umwelt e.V. dormakaba International Holding GmbH
Hegelplatz 1 DORMA Platz 1
10117 Berlin 58256 Ennepetal
Germany Germany
Declaration number Declared product / declared unit
EPD­DOR­20210083­IBI1­EN The declared unit is one piece of the ST PRO Green RC automatic sliding
door system comprising:
• representative value of the ES PROLINE drive system
• two sliding panels
• respective packaging materials
The LCA results for two side screens and a fanlight are presented in the
appendix.
This declaration is based on the product category rules: Scope:
Automatic doors, automatic gates, and revolving door systems, This EPD refers to the entire life cycle of a DORMA ST PRO Green RC
01/08/2021 automatic sliding door system.
(PCR checked and approved by the SVR) The various technical characteristics are outlined in section 2.3. The
production location is dormakaba Zusmarshausen, Germany. Product
components are also procured from the DORMA facilities in Ennepetal.
Issue date The material and energy flows were taken into consideration accordingly.
The owner of the declaration shall be liable for the underlying information
28/06/2021
and evidence; the IBU shall not be liable with respect to manufacturer
information, life cycle assessment data and evidences.
Valid to
The EPD was created according to the specifications of EN 15804+A1. In
27/06/2026 the following, the standard will be simplified as EN 15804 bezeichnet.
Verification
The standard EN 15804 serves as the core PCR
Independent verification of the declaration and data according to ISO
14025:2011
internally X externally
Dipl.­Ing Hans Peters
(chairman of Institut Bauen und Umwelt e.V.)
Florian Pronold Dr.­Ing. Wolfram Trinius,
(Managing Director Institut Bauen und Umwelt e.V.) (Independent verifier)
1 Environmental­Product Declaration ­ dormakaba Deutschland GmbH ­ ST PRO Green RC
2. Product
2.1 Product description/Product definition
The ST PRO Green RC convinces due to its strengthened
profile system and safety. The ST PRO Green RC is tested and
certified by ift Rosenheim. A continuous floor rail in the door leaf
area and a sabotage protection in the drive prevent the door
wings from being levered out.
Additional safety is guaranteed due to a multi­point hook
locking in the area of the main closing edge.
The door variant is equipped with a hook on the secondary
closing edge and burglar­resistant glazing.
The slim profile system can be used with double­ and triple
glazing, whereby UD values of down to 1.0 W/(m²·K) (glass
heat transfer coefficient) can be realized.
Together with the thermally separated profile the energy losses
are minimized
Thanks to the new ES PROLINE drive system single door
leaves up to 250kg and double door leaves up to 200kg each
can be moved quickly and quietly.
The low energy consumption of the sliding door drive also 2.3 Technical Data
contributes to the overall energy efficiency of the sliding door
Technical data of the ES 400 PRO drive system used for ST
system.
PRO Green RC standard and emergency exit sliding doors
The drive is suitable for almost all sliding door applications,
Constructional data ES PROLINE
including use on escape route sliding doors. For the placing on Name Value Unit
the market in the European Union/European Free Trade Height mm 100
Associaton (EU/EFTA) (with the exception of Switzerland) the
Installation depth mm 180
following legal provisions apply:
Opening and closing force N 150
• Machinery Directive 2006/42/EC
Opening speed ES 400 PRO cm/s 10­90
• 2014/30/EU Electromagnetic Compatibility Directive
Opening speed ES 400 PRO FST cm/s 20­90
• 2011/65/EU ROHS3 Directive
• DIN EN ISO 12100:2011-03 Safety of machinery Closing speed ES 400 PRO cm/s 10­90
• DIN EN 16005: 2013-01 and Amendment 2015-10 Hold open time ES PROLINE s 0­180
Power operated pedestrian doorsets Supply voltage, frequency ES PROLINE Hz 50­60
• DIN EN ISO 13849- 1:2016-06 Safety of machinery
Power input ES PROLINE W 130­180
• DIN EN 60335-2-103: 2016-05 Household and similar
Protection type IP ­ 120
electrical appliance
Low­voltage and EMC Directives ­ ­
• DIN EN 61000-3-2:2015-03 Electromagnetic
compatibility (EMC) Product not harmonised in accordance with the CPR but in
• DIN EN 61000­3­3: 2014­03 Electromagnetic accordance with other provisions for harmonisation of the EU:
compatibility (EMC)
• Machinery Directive 2006/42/EC
• DIN EN 61000-6-2: 2005 and Amendment:2011
• 2014/30/EU Electromagnetic Compatibility Directive
Electromagnetic Compatibility (EMC)
• 2011/65/EU ROHS3 Directive
• DIN EN 61000-6-3:2007 and A1:2011 Electromagnetic
Compatibility (EMC) 2.4 Delivery status
• DIN EN IEC 63000: 2019-05
As an automatic sliding door involves a customised door
The CE­marking takes into account the proof of conformity with
system, shapes and sizes can vary considerably. The ST PRO
the respective harmonized standards based on the legal
Green RC under review has the following delivery status:
provisions above.
2.2 Application
With the ST PRO Green RC sliding door profile system both
standard sliding doors and escape route sliding doors can be
equipped by using the ES 400 PRO drive system:
The components associated with these dimensions have the
following weights:
2 Environmental­Product Declaration ­ dormakaba Deutschland GmbH ­ ST PRO Green RC
Waste air generated during production is cleaned in
accordance with statutory specifications. Emissions are
significantly below the Technical Instructions on Air Quality.
Water/Ground:
No contamination of water or ground.
Production ­related waste/ water is treated internally and
redirected to the production process.
Sound protection:
The ES PROLINE operator systems are supplied in a separate Analyses have established that all values communicated inside
box; the sliding panels and side screens are supplied on and outside the production facilities are far below the standards
frames. applicable in Germany.
The Environmental Management system in the dormakaba
2.5 Base materials/Ancillary materials
production facility Ennepetal and Zusmarshausen is certified to
Mass percentages of the automatic sliding door system: ISO 14001; industrial safety is certified to OHSAS 18001.
2.8 Product processing/Installation
The product system is installed by specially­trained assembly
teams.
2.9 Packaging
The declared unit comprises the following packaging
materials and their mass percentages:
The products include partial articles which contain substances
listed in the candidate list of REACH Regulation 1907/2006/EC
(date: 19.01.2021) exceeding 0.1 percentage by mass: yes
• Lead (Pb): 7439­92­1 (CAS­No.) is
included in some of the alloys used. The concentration More
of lead in each information on the possible disposal is provided in section 2.14
individual alloy does not exceed 4.0% (by mass). and
2.15.
This product/article/at least one partial article contains
other carcinogenic, mutagenic, reprotoxic (CMR) substances in 2.10 Condition of use
categories 1A or 1B which are not on the candidate list, No auxiliaries
exceeding 0.1 percentage by mass: no. or consumables are incurred during maintenance, and use of
the sliding door system ST PRO Green RC. Regular
Biocide products were added to this construction product or it maintenance is advised to ensure the service life of 15 years.
has been treated with biocide products (this then concerns a
treated product as defined by the (EU) Ordinance on Biocide For repairs or renewals, suitable spare parts are available. The
Products No. 528/2012): no. energy supply
for the analysed sliding door has been calculated for the
2.6 Manufacture
reference service life
The ST PRO Green RC sliding panels and side screens are of 15 years.
manufactured in the DORMA plant Zusmarshausen. The ES
PROLINE drive units 2.11 Environment and health during use
and requisite circuit boards are manufactured at There are no
dormakaba. The certified Quality Management system in known impact relations between product, environment and
accordance with ISO 9001 safeguards the high health during use.
quality standard of dormakaba products. It guarantees
continuous improvement of 2.12 Reference service life
the overall processes and product quality at the The declaration of the reference service life (RSL) is imperative
dormakaba locations. for EPDs covering the complete use stage (modules B1­B7), or
if a use stage scenario is described, which refers to the lifetime
2.7 Environment and health during manufacturing of the product. If not all modules of the use stage are declared
No health protection measures beyond the legally specified and no use stage scenario covering the full lifetime of the
measures are required. The maximum allowable concentrations product is described, then the indication of the RSL (according
are clearly complied with at each point of production. to ISO 15686:1, -2, -7 and -8) is voluntary.
Air:
3 Environmental­Product Declaration ­ dormakaba Deutschland GmbH ­ ST PRO Green RC
Information on the product’s RSL requires specification of No impacts on the environment are expected in the case of an
compatible scenarios for the product stage, construction unforeseeable mechanical destruction.
process stage and use stage. The RSL is dependent on the
properties of the prod¬uct and reference in­use conditions. 2.14 Re-use phase
These conditions shall be declared together with the RSL in With reference to the material composition of the product
clause 4 and it shall be stated that the RSL applies for the system in accordance with section 2.5, the following
reference conditions only. possibilities arise:
If a reference service life (RSL) cannot be declared according Re-use
to ISO 15686 (or it is not relevant for consideration of the LCA), During refurbishment or deconstruction, sliding doors can be
this has to be stated clearly in the EPD. easily segregated and reused for the same application.
In such cases, a service life can be declared in ac­cordance Material recycling
with the BBSR table "Service lives of components for life cycle The metallurgical materials and glass contained in the product
assessment according to are suitable for material recycling.
BNB" (www.nachhaltigesbauen.de/baustoff­und­
gebaeudedaten/nutzungsdauern­von­bauteilen.html). Energy recovery
The plastics contained in the product are suitable for energetic
It shall be unambiguously stated that a service life (not: a recovery.
reference service life) in accordance with the BBSR table (or
based on a manufacturer’s declaration (see below)) is not a Landfilling
RSL according to ISO 15686. Is not applicable.
A service life provided by the manufacturer can be declared as 2.15 Disposal
an alternative to the value from the BBSR table. This Cuttings:
information shall be accompanied by explanations on the origin Cuttings incurred during the manufacturing phase are directed
of the declared service life, e.g. referring to simulations, tests, towards metallurgical recycling and energy recovery. Cuttings
an assessment of the man¬ufacturer or statistical data, etc. and are collected separately and collected by a disposal company.
shall contain the specification of the application for which the Following European Waste Catalogue (EWC) Codes are
stated service life is valid (to be provided in clause 4). relevant:
• EWC 07 02 03 Plastic waste
The requisite information for technical building installations • EWC 12 01 01 Ferrous metal filings and turnings
should be taken from VDI 20673. • EWC 12 01 03 Non­ferrous metal filings and turnings
Packaging:
The reference
Packaging incurred for installation in the building is directed
service life amounts to 15 years. This complies with 1,500,000
towards energy recovery.
cycles according
• EWC 15 01 01 Paper and cardboard packaging
to EN 16005.
• EWC 15 01 02 Plastic packaging
2.13 Extraordinary effects End of Life:
Fire All materials contained in the product are directed to energy
Due to the predominant use of recovery or recycling process.
aluminium and steel which are considered non­flammable or • EWC 16 02 14 Used devices with the exception of those
flame­retardant, no additional influence on the environment in included in 16 02 09 to 16 02 1
case of fire is to be expected. • EWC 16 02 16 Components removed from used
Fire protection devices with the exception of those included in 16 02 15
• EWC 17 02 03 Plastic
Name Value
• EWC 17 04 02 Aluminum
Building material class not applicable
• EWC 17 04 05 Iron and steel
Burning droplets not applicable • EWC 17 04 11 Cables with the exception of those
Smoke gas development not applicable included in 17 04 10
• EWC 17 02 02 Glass
Water 2.16 Further information
No substances are used which have a negative impact on the
Contact data for more detailed information:
ecological water quality upon contact by the device with water.
Please refer to the last page of this Declaration
Mechanical destruction
3. LCA: Calculation rules
Name Value Unit
3.1 Declared Unit
Declared unit for automatic doors and gates 4.07 m2
The declared unit is one (1) piece ST PRO Green RC. The
declared unit consists of the drive system and two sliding Grammage 56.03 kg/m2
panels. The results for two side screens and a fanlight are Mass (total system) 228.08 kg
presented in the appendix. Conversion factor to 1 kg 0.004 ­
Declared unit
For IBU core EPDs (where clause 3.6 is part of the EPD): for
average EPDs, an estimate of the robustness of the LCA
values must be made, e.g. concerning variability of the
4 Environmental­Product Declaration ­ dormakaba Deutschland GmbH ­ ST PRO Green RC
production process, geographical representativeness and the specific data.
influence of background data and preliminary products However, generic background datasets were used for
compared to the environmental impacts caused by actual the upstream and downstream processes. The majority
production. of the background datasets used were taken from the
current version of the GaBi 10.0 database. Ecoinvent Version
3.6 and Ecoinvent Version 2.2 datasets were only used when
3.2 System boundary
suitable GaBi 10.0 datasets were not available.
Type of the EPD: cradle to gate ­ with options
Modules A1-A3, A4, and A5 Where possible, German datasets were used for modules A1­
The product stage (A1­A3) begins with considering the A3, and the corresponding European datasets for distribution
production of the necessary raw materials and energies, transports (A4), installation (A5) and disposal scenarios (C
including all corresponding upstream chains and the actual modules).
procurement transports. Furthermore, the entire manufacturing
phase was mapped, including the treatment of production 3.6 Data quality
waste until the end­of­waste status (EoW) was reached. In The background datasets used for accounting purposes mainly
addition, both the distribution transports (A4) and the originate from the respective updated GaBi 10.0 databases at
installation including power­consuming tools, installation the time of calculation.
materials and the packaging waste generated during
installation (A5) were taken into account. The data for the examined products was captured on the basis
of evaluations of internal production and environmental data,
Module B6 the collection of LCA­­relevant data within the supply chain, as
Module B6 includes the operational energy use over the well as the evaluation of relevant data for the energy supply.
Reference Service Life of 15 years. The collected data were checked for plausibility and
consistency. Good representativity can be assumed.
Modules C1-C4
The modules include the environmental impacts for dismantling 3.7 Period under review
of the ST PRO Green RC and the treatment of the waste Life cycle assessment data were collected in 2019 and 2020.
categories until end­of­waste status (EoW) is reached, including
3.8 Geographic Representativeness
the associated transports at the end of the product life cycle.
Land or region, in which the declared product system is
Module D manufactured, used or handled at the end of the product´s
Identification of the benefits and costs of the product outside lifespan: Germany
the system boundary. For plastics, these consist of energy
credits from thermal utilization (C3) in the form of the average
3.9 Allocation
European electricity mix or thermal energy from natural gas.
All required energies, raw materials, and supplies could be
Recycling of glass and metal scrap results in credits of the
clearly assigned to the declared product. No by­­products are
respective raw materials.
produced and no allocation is required. In module A1­­A3,
3.3 Estimates and assumptions credits are issued for recycling of metallurgical waste.
Packaging materials and the combustible product parts are
It was assumed that End of Life thermal waste incineration
incinerated at the end of life in a waste incineration plant.
plants are plants with an R1 factor (energy conversion
Metallurgical parts and glass are recycled. Any emissions that
efficiency or energy efficiency of waste incineration plants
occur are taken into account in the model. Depending on their
according to the European Waste Framework Directive) >0.6.
elementary composition and the resulting heating values,
3.4 Cut-off criteria recycling credits are taken into account in module D.
The effect associated with the neglected mass shares is less
3.10 Comparability
than 5% of the effect categories per module. The minimum limit
Basically, a comparison or an evaluation of EPD data is only
of 1% total mass and the use of renewable and non­renewable
possible if all the data sets to be compared were created
primary energy is not exceeded.
according to EN 15804 and the building context, respectively
3.5 Background data the product­specific characteristics of performance, are taken
The LCA software GaBi 10.0 was used to model the life cycle. into account.
The entire manufacturing process, as well as energy The used background database has to be mentioned.
consumption, were modelled on the basis of manufacturer­
4. LCA: Scenarios and additional technical information
materials included in the LCA calculations must be declared as
The following technical scenario information is required for the technical scenario information for Module A5.
declared modules and optional for non­declared modules.
Modules for which no information is declared can be deleted;
additional information can also be listed if necessary.
Transport to the building site (A4)
Name Value Unit
The following technical information is a basis for the declared
modules or can be used for developing specific scenarios in the Litres of fuel unknown l/100km
context of a building assessment if modules are not declared Transport distance (Truck) 525 km
(MND). Capacity utilisation (including empty runs) 55 %
Gross density of products transported unknown kg/m3
A5 is not declared including the disposal of the packaging
Capacity utilisation volume factor unknown ­
material on the construction site, the amounts of packaging
5 Environmental­Product Declaration ­ dormakaba Deutschland GmbH ­ ST PRO Green RC
Name Value Unit
Collected separately waste type waste type 228.24 kg
Installation into the building (A5) Collected as mixed construction waste ­ kg
Name ValueUnit Reuse ­ kg
Auxiliary 0.155 kg Recycling 215.73 kg
Electricity consumption 0.04 kWh Energy recovery 12.51 kg
Output substances following waste treatment on Landfilling ­ kg
3 kg
site (packaging materials)
Reference service life Reuse, recovery and/or recycling potentials (D), relevant
Name Value Unit scenario information
Life Span according to the manufacturer 15 a Name Value Unit
Net steel scrap 15.04 kg
Operational energy use (B6) and Operational water use
Net aluminium scrap 8.59 kg
(B7)
Net zinc scrap 1.5 kg
Name Value Unit
Collection rate 100 %
Electricity consumption 988.49 kWh
Recycling loss 0 %
End of life (C1-C4)
6 Environmental­Product Declaration ­ dormakaba Deutschland GmbH ­ ST PRO Green RC
5. LCA: Results
The following table shows the results of the LCA for 1 piece declared ST PRO Green RC. The results in module B6 are based on a
lifetime of 15 years. The LCA results for two side screens and a fanlight are presented in the appendix.
DESCRIPTION OF THE SYSTEM BOUNDARY (X = INCLUDED IN LCA; MND = MODULE NOT DECLARED; MNR = MODULE NOT
RELEVANT)
BENEFITS
AND LOADS
CONSTRUCTION
BEYOND
PRODUCT STAGE PROCESS USE STAGE END OF LIFE STAGE
THE SYSTEM
STAGE
BOUNDARIE
S
la ire ta m w a Ry lp p u s tro p s n a rT g n iru tc a fu n a M e h t m o rf tro p s n a rTe tis e h t o t e ta g y lb m e s s A e s U e c n a n e tn ia M ria p e R tn e m e c a lp e R tn e m h s ib ru fe R y g re n e la n o ita re p Oe s u re ta w la n o ita re p Oe s u n o itc u rts n o c ­e Dn o itilo m e d tro p s n a rT g n is s e c o rp e ts a W la s o p s iD ­e s u e R­y re v o c e R­g n ilc y c e Rla itn e to p
A1 A2 A3 A4 A5 B1 B2 B3 B4 B5 B6 B7 C1 C2 C3 C4 D
X X X X X MND MND MNR MNR MNR X MND X X X X X
RESULTS OF THE LCA - ENVIRONMENTAL IMPACT according to EN 15804+A1: 1 piece ST PRO Green RC
Parameter Unit A1-A3 A4 A5 B6 C1 C2 C3 C4 D
GWP kg CO 2 eq 8.44E+02 1E+01 4.99E+00 3.9E+02 8.22E­03 6.9E­01 3.15E+01 0 ­1.3E+02
ODP kg CFC11 eq 1.23E­05 1.65E­15 5.95E­15 1.17E­11 2.46E­16 2.17E­16 1.64E­07 0 ­4.84E­08
AP kg SO 2 eq 5.28E+00 4.23E­02 2.23E­03 8.19E­01 1.73E­05 2.94E­03 1.96E­02 0 ­5.37E­01
EP kg PO 43 eq 9.82E­01 1.06E­02 3.36E­04 9.06E­02 1.91E­06 7.34E­04 1.79E­02 0 ­5.69E­02
POCP kg Ethen eq 3.24E­01 ­1.78E­02 2.01E­04 5.83E­02 1.23E­06 ­1.1E­03 1.56E­03 0 ­4.08E­02
ADPE kg Sb eq 6.49E­02 8.34E­07 2.35E­05 1.3E­04 2.75E­09 6.49E­08 6.3E­05 0 ­6.29E­03
ADPF MJ 1.12E+04 1.37E+02 9.73E+00 4.32E+03 9.11E­02 9.42E+00 3.04E+01 0 ­1.48E+03
GWP = Global warming potential; ODP = Depletion potential of the stratospheric ozone layer; AP = Acidification potential of land and water; EP =
Eutrophication potential; POCP = Formation potential of tropospheric ozone photochemical oxidants; ADPE = Abiotic depletion potential for non­fossil
resources; ADPF = Abiotic depletion potential for fossil resources
RESULTS OF THE LCA - INDICATORS TO DESCRIBE RESOURCE USE according to EN 15804+A1: 1 piece ST PRO Green RC
Parameter Unit A1-A3 A4 A5 B6 C1 C2 C3 C4 D
PERE MJ 2.12E+03 7.7E+00 3.91E+01 3.1E+03 6.53E­02 5.51E­01 4.56E+00 0 ­4.45E+02
PERM MJ 3.77E+01 0 ­3.77E+01 0 0 0 0 0 0
PERT MJ 2.16E+03 7.7E+00 1.36E+00 3.1E+03 6.53E­02 5.51E­01 4.56E+00 0 ­4.45E+02
PENRE MJ 1.3E+04 1.37E+02 1.08E+01 7E+03 1.47E­01 9.46E+00 3.15E+02 0 ­1.67E+03
PENRM MJ 2.81E+02 0 ­3.44E­01 0 0 0 ­2.8E+02 0 0
PENRT MJ 1.33E+04 1.37E+02 1.05E+01 7E+03 1.47E­01 9.46E+00 3.44E+01 0 ­1.67E+03
SM kg 5.01E+01 0 0 0 0 0 0 0 1.66E+02
RSF MJ 0 0 0 0 0 0 0 0 0
NRSF MJ 0 0 0 0 0 0 0 0 0
FW m3 1.01E+01 8.92E­03 1.41E­02 3.59E+00 7.56E­05 5.95E­04 9.3E­02 0 ­4.32E+00
PERE = Use of renewable primary energy excluding renewable primary energy resources used as raw materials; PERM = Use of renewable primary
energy resources used as raw materials; PERT = Total use of renewable primary energy resources; PENRE = Use of non­renewable primary energy
excluding non­renewable primary energy resources used as raw materials; PENRM = Use of non­renewable primary energy resources used as raw
materials; PENRT = Total use of non­renewable primary energy resources; SM = Use of secondary material; RSF = Use of renewable secondary fuels;
NRSF = Use of non­renewable secondary fuels; FW = Use of net fresh water
RESULTS OF THE LCA – WASTE CATEGORIES AND OUTPUT FLOWS according to EN 15804+A1:
1 piece ST PRO Green RC
Parameter Unit A1-A3 A4 A5 B6 C1 C2 C3 C4 D
HWD kg 1.15E­01 6.38E­06 2.41E­08 2.9E­06 6.1E­11 4.12E­07 5.24E­08 0 ­2.78E­06
NHWD kg 2.81E+02 2.1E­02 1.39E­01 4.96E+00 1.05E­04 1.56E­03 3.21E+00 0 ­2E+01
RWD kg 6.79E­01 1.7E­04 3.15E­04 1.06E+00 2.24E­05 1.6E­05 5.49E­04 0 ­7.71E­02
CRU kg 0 0 0 0 0 0 0 0 0
MFR kg 9.64E+00 0 0 0 0 0 2.13E+02 0 0
MER kg 3.01E+00 0 2.98E+00 0 0 0 1.48E+01 0 0
EEE MJ 0 0 6.57E+00 0 0 0 5.28E+01 0 0
EET MJ 0 0 1.19E+01 0 0 0 1.11E+02 0 0
HWD = Hazardous waste disposed; NHWD = Non­hazardous waste disposed; RWD = Radioactive waste disposed; CRU = Components for re­use;
MFR = Materials for recycling; MER = Materials for energy recovery; EEE = Exported electrical energy; EET = Exported thermal energy
6. LCA: Interpretation
7 Environmental­Product Declaration ­ dormakaba Deutschland GmbH ­ ST PRO Green RC
The CML characterization factors were used for the evaluation. Acidification potential (AP) in modules A1­A3 is dominated by
The results of the CML categories refer to the potential the glass (66%) and the operator (22%).
environmental impacts over a period of 100 years. Eutrophication potential (EP) in modules A1­A3 is dominated by
The main impacts lie in the modules A1­A3 and B6. The the operator (65%) and there the electronic components. The
impacts in module B6 are due to the electricity mix used for glass also has a significant impact on the EP (29%).
modelling the electricity consumption over a period of 15 years. Formation potential of tropospheric ozone photochemical
In the following, the main influences on the modules A1­A3 for oxidants (POCP) in modules A1­A3 is mainly influenced by the
the indicators will be explained. glass.
Abiotic depletion potential for non­­fossil resources in modules
Global warming potential (GWP) in modules A1­A3 is mainly A1­A3 is dominated by the operator (91%) and there the
influenced by the glass (43%), the operator (25%) and electronic components.
aluminium (20%). Abiotic depletion potential for fossil resources (ADPF) in
Ozone depletion potential in module A1­A3 is mainly influenced modules A1­A3 is dominated by the glass (52%).
by the electronic components of the operator (>90%).
7. Requisite evidence
8. References
Standards EN 61000-3-2
DIN EN 61000­3­2:2015­03, Electromagnetic compatibility
EN 15804 (EMC) ­ Part 3­2:
EN 15804:2012­04+A1 2013, Sustainability of construction Limits ­ Limits for harmonic current emissions (equipment input
works — Environmental Product Declarations — Core rules for current ≤ 16 A per phase).
the product category of construction products.
EN 16005 EN 61000-3-3
DIN EN 16005:2013­01 and Amendment 2015­10, Power DIN EN 61000­3­3:2014­03, Electromagnetic compatibility
operated pedestrian doorsets ­ Safety in use ­ Requirements (EMC) ­ Part 3­3:
and test methods. Limits ­ Limitation of voltage changes, voltage fluctuations and
flicker in public low­voltage supply systems, for equipment with
rated current ≤ 16 A per phase and not subject to conditional
EN 60335-2-103 connection.
DIN EN 60335­2­103:2016­05, Household and similar electrical
appliances ­ Safety ­ Part 2­103: Particular requirements for
drives for gates, doors and windows. EN 61000-6-2
DIN EN 61000­6­2:2005 + Amendment:2011. Electromagnetic
compatibility (EMC) ­ Part 6­2: Generic standards ­ Immunity
standard for industrial environments.
8 Environmental­Product Declaration ­ dormakaba Deutschland GmbH ­ ST PRO Green RC
Council of 8 June 2011 on the restriction of the use of certain
EN 61000-6-3 hazardous substances in electrical and electronic equipment
DIN EN 61000­6­3:2007 + A1:2011, Electromagnetic 2014/30/EU Electromagnetic Compatibility Directive
compatibility (EMC) ­ Part 6­3: Generic standards ­ Emission Directive 2014/30/EU of the European Parliament and of the
standard for residential, commercial and light­industrial Council of 26 February 2014 on the harmonisation of the laws
environments. of the Member States relating to electromagnetic compatibility
(recast) CML
Institute of Environmental Sciences Leiden University
IEC 63000 Ecoinvent Version 2.2
DIN EN IEC 63000:2019­05, Technical documentation for the Database for life cycle assessment (life cycle inventory data),
assessment of electrical and electronic products with respect to Version 2.2, 2010.
the restriction of hazardous substances. Ecoinvent Version 3.6
Database for life cycle assessment (life cycle inventory data),
Version 3.6, 2019.
ISO 9001 EWC
DIN EN ISO 9001:2015­11, Quality management systems ­ European Waste Catalogue (EWC). Commission Decision on
Requirements (ISO 9001:2015); German and English version the European List of Waste (COM 2000/532/EC) GaBi 10.0
EN ISO 9001:2015 Life cycle engineering (GaBi) software and database. LBP,
University of Stuttgart and thinkstep AG, Documentation of
GaBi 10.0 data sets http://documentation.gabisoftware.com/,
ISO 12100 2020.
DIN EN ISO 12100:2011­03, Safety of machinery ­ General IBU 2016
principles for design ­ Risk assessment and risk reduction. Institut Bauen und Umwelt e.V.: General Programme
Instructions for the Preparation of EPDs at the Institut Bauen
und Umwelt e.V. Version 1., Berlin: Institut Bauen und Umwelt
ISO 13849-1 e.V., 2016. www.ibu­epd.com IP
DIN EN ISO 13849­1:2016­06, Safety of machinery ­ Safety­ Ingress Protection Rating. DIN EN 60529; VDE 04701: 201409:
related parts of control systems ­ Part 1: General principles for Degrees of protection provided by enclosures (IP Code) (IEC
design. 60529:1989 + A1:1999 + A2:2013); German version EN
ISO 14001 60529:1991 + A1:2000 + A2:2013 Machinery Directive
2006/42/EC
ISO 14001:2015­09, Environmental management systems ­ Directive 2006/42/EC of the European Parliament and of the
Requirements with guidance for use ISO 14025 Council of 17 May 2006 on machinery, and amending Directive
95/16/EC (recast) Ordinance on Biocide Products No.
DIN EN ISO 14025:2011­10, Environmental labels and 528/2012
declarations — Type III environmental declarations — Regulation (EU) No 528/2012 of the European Parliament and
Principles and procedures. of the Council of 22 May 2012 concerning the making available
OHSAS 18001 on the market and use of biocidal products Product Category
Rules Part A
Occupational health and safety – Management systems – Calculation Rules for the Life Cycle Assessment and
Requirements Requirements on the Project Report. Version 1.8 (04.07.2019)
Further references Product Category Rules Part B
Requirements on the EPD for Automatic doors, automatic
2011/65/EU ROHS3 Directive gates, and revolving door systems. Version 1.1 (09.07.2013)
Directive 2011/65/EU of the European Parliament and of the
9 Environmental­Product Declaration ­ dormakaba Deutschland GmbH ­ ST PRO Green RC
Publisher
Institut Bauen und Umwelt e.V. +49 (0)30 3087748­ 0
Hegelplatz 1 info@ibu­epd.com
10117 Berlin www.ibu­epd.com
Germany
Programme holder
Institut Bauen und Umwelt e.V. +49 (0)30 3087748­ 0
Hegelplatz 1 info@ibu­epd.com
10117 Berlin www.ibu­epd.com
Germany
Author of the Life Cycle Assessment
brands & values GmbH +49 421 70 90 84 33
Altenwall 14 info@brandsandvalues.com
28195 Bremen www.brandsandvalues.com
Germany
Owner of the Declaration
dormakaba International Holding GmbH +49 2333 793­0
DORMA Platz 1 info.de@dormakaba.com
58256 Ennepetal www.dormakaba.com
Germany
10 Environmental­Product Declaration ­ dormakaba Deutschland GmbH ­ ST PRO Green RC
