ENVIRONMENTAL-PRODUCT DECLARATION
as per ISO 14025 and EN 15804+A1
Owner of the Declaration dormakaba International Holding GmbH
Publisher Institut Bauen und Umwelt e.V. (IBU)
Programme holder Institut Bauen und Umwelt e.V. (IBU)
Declaration number EPD-DOR-20210082-IBI1-EN
Issue date 28.06.2021
Valid to 27.06.2026
ST PRO Green
dormakaba
www.ibu-epd.com | https://epd-online.com
1. General Information
dormakaba ST PRO Green
Programme holder Owner of the declaration
IBU – Institut Bauen und Umwelt e.V. dormakaba International Holding GmbH
Hegelplatz 1 DORMA Platz 1
10117 Berlin 58256 Ennepetal
Germany Germany
Declaration number Declared product / declared unit
EPD­DOR­20210082­IBI1­EN The declared unit is one piece of the ST PRO Green automatic sliding door
system comprising:
• representative value of the ES PROLINE drive system
• two sliding panels
• respective packaging materials.
The LCA results for two side screens and a fanlight are presented in the
appendix.
This declaration is based on the product category rules: Scope:
Automatic doors, automatic gates, and revolving door systems, This EPD refers to the entire life cycle of a DORMA ST PRO GREEN
01.08.2021 automatic sliding door system.
(PCR checked and approved by the SVR)
The various technical characteristics are outlined in section 2.3. The
production location is dormakaba Zusmarshausen, Germany. Product
Issue date components are also procured from the DORMA facilities in Ennepetal.
The material and energy flows were taken into consideration accordingly.
28.06.2021
The owner of the declaration shall be liable for the underlying information
and evidence; the IBU shall not be liable with respect to manufacturer
information, life cycle assessment data and evidences.
Valid to
27.06.2026 The EPD was created according to the specifications of EN 15804+A1. In
the following, the standard will be simplified as EN 15804 bezeichnet.
Verification
The standard EN 15804 serves as the core PCR
Independent verification of the declaration and data according to ISO
14025:2011
internally X externally
Dipl.­Ing Hans Peters
(chairman of Institut Bauen und Umwelt e.V.)
Florian Pronold Dr.­Ing. Wolfram Trinius,
(Managing Director Institut Bauen und Umwelt e.V.) (Independent verifier)
1 Environmental­Product Declaration ­ dormakaba ­ ST PRO Green
2. Product
2.1 Product description/Product definition 2.3 Technical Data
The ST PRO GREEN convinces with its comprehensive energy Technical data of the ES PROLINE drive systems used for ST
efficiency: PRO GREEN standard and emergency exit sliding doors
Constructional data ES PROLINE
The slim profile system can be used with double and triple
Name Value Unit
glazing, whereby UD values of down to 1.0 W/(m²·K) (glass
heat transfer coefficient) can be realized. Height mm 100
Together with the thermally separated profile the energy losses Installation depth 180 mm 180
are minimized. Opening and closing force 150 N 150
Opening speed ES 250 PRO 10­70 cm/s 10­70
Thanks to the new ES PROLINE drive system single door
Opening speed ES 400 PRO 10­90 cm/s 10­90
leaves up to 250kg and double door leaves up to 200kg each
can be moved quickly and quietly. Opening speed ES 250 PRO Easy 10­70 cm/s 10­70
The low energy consumption of the sliding door drive also Opening speed ES 250 PRO FST 20­70 cm/s 20­70
contributes to the overall energy efficiency of the sliding door Opening speed ES 400 PRO FST 20­90 cm/s 20­90
system.
Closing speed ES 250 PRO 10­70 cm/s 10­70
The drive is suitable for almost all sliding door applications,
Closing speed ES 400 PRO 10­90 cm/s 10­90
including use on escape route sliding doors. For the placing on
the market in the European Closing speed ES 250 PRO Easy 10­70 cm/s 10­70
Hold open time ES PROLINE 0­180 s 0­180
Union/European Free Trade Associaton (EU/EFTA) Supply voltage, frequency ES PROLINE 50­60 Hz 50­60
Power input ES PROLINE 130­180 W 130­180
(with the exception of Switzerland) the following legal
Protection type IP 120 ­ 120
Low­voltage and EMC Directives ­ ­ ­
provisions apply:
• Machinery Directive 2006/42/EC Product not harmonised in accordance with the CPR but in
• 2014/30/EU Electromagnetic Compatibility Directive accordance with other provisions for harmonisation of the EU:
• 2011/65/EU ROHS3 Directive • Machinery Directive 2006/42/EC
• DIN EN ISO 12100:2011-03 Safety of machinery • 2014/30/EU Electromagnetic Compatibility Directive
• DIN EN 16005: 2013-01 and Amendment 2015-10 • 2011/65/EU ROHS3 Directive
Power operated pedestrian doorsets
• DIN EN ISO 13849- 1:2016-06 Safety of machinery 2.4 Delivery status
• DIN EN 60335-2-103: 2016-05 Household and similar As an automatic sliding door involves a customised door
electrical appliance system, shapes and sizes can vary considerably. The ST PRO
• DIN EN 61000-3-2:2015-03 Electromagnetic Green under review has the following delivery status:
compatibility (EMC)
• DIN EN 61000­3­3: 2014­03 Electromagnetic
compatibility (EMC)
• DIN EN 61000-6-2: 2005 and Amendment:2011
Electromagnetic Compatibility (EMC)
• DIN EN 61000-6-3:2007 and A1:2011 Electromagnetic
Compatibility (EMC)
• DIN EN IEC 63000: 2019-05
The CE­marking takes into account the proof of conformity with
the respective harmonized standards based on the legal
provisions above.
2.2 Application
The components associated with these dimensions have the
With the sliding door profile system both standard sliding doors following weights:
and escape route sliding doors can be equipped. Following
automatic ES PROLINE drive system can be used:
The ES PROLINE automatic drive system is supplied in a
separate box; the sliding panels and side screens are supplied
on frames.
2.5 Base materials/Ancillary materials
2 Environmental­Product Declaration ­ dormakaba ­ ST PRO Green
Mass percentages of the automatic sliding door system:
2.9 Packaging
The declared unit comprises the following packaging materials
and their mass percentages:
More information on the possible disposal of packaging is
provided in section 2.14 and 2.15.
The products include partial articles which contain substances 2.10 Condition of use
listed in the candidate list of REACH Regulation 1907/2006/EC
No auxiliaries or consumables are incurred during
(date: 19.01.2021) exceeding 0.1 percentage by mass: yes
maintenance, and use of the sliding door system ST PRO
• Lead (Pb): 7439­92­1 (CAS­No.) is included in some of GREEN. Regular maintenance
the alloys used. The concentration of lead in each
individual alloy does not exceed 4.0% (by mass). is advised to ensure a service life of 15 years.
This product/article/at least one partial article contains other
carcinogenic, mutagenic, reprotoxic (CMR) substances in For repairs or renewals, suitable spare parts are available. The
categories 1A or 1B which are not on the candidate list, energy supply for the analysed sliding door has been calculated
exceeding 0.1 percentage by mass: no. for the reference service life of 15 years.
Biocide products were added to this construction product or it 2.11 Environment and health during use
has been treated with biocide products (this then concerns a There are no known impact relations between product,
treated product as defined by the (EU) Ordinance on Biocide environment and health during use.
Products No. 528/2012): no.
2.12 Reference service life
2.6 Manufacture The reference service life amounts to 15 years. This complies
The ST PRO Green sliding panels and side screens are with 1,500,000 cycles according to EN 16005.
manufactured in the DORMA plant Zusmarshausen. The ES
2.13 Extraordinary effects
PROLINE drive units and requisite circuit boards are
manufactured at dormakaba. The certified Quality Management Fire
system in accordance with ISO 9001 safeguards the high Due to the predominant use of aluminium and steel which are
quality standard of dormakaba products. It guarantees considered non­flammable or flame­retardant, no additional
continuous improvement of the overall processes and product influence on the environment in case of fire is to be expected.
quality at the dormakaba locations. Fire protection
Name Value
2.7 Environment and health during manufacturing
No health protection measures beyond the legally specified Building material class not applicable
measures are required. The maximum allowable concentrations Burning droplets not applicable
are clearly complied with at each point of production. Smoke gas development not applicable
Air:
Water
Waste air generated during production is cleaned in
No substances are used which have a negative impact on the
accordance with statutory specifications. Emissions are
ecological water quality upon contact by the device with water.
significantly below the Technical Instructions on Air Quality.
Mechanical destruction
Water/Ground:
No impacts on the environment are expected in the case of an
No contamination of water or ground. Production­related
unforeseeable mechanical destruction.
waste/water is treated internally and redirected to the
production process. 2.14 Re-use phase
With reference to the material composition of the product
Sound protection:
system in accordance with section 2.5, the following
Analyses have established that all values communicated inside
possibilities arise:
and outside the production facilities are far below the standards
applicable in Germany.
Re-use
The Environmental Management system in the dormakaba
During refurbishment or deconstruction, sliding doors can be
production facility Ennepetal and Zusmarshausen is certified to
easily segregated and reused for the same application.
ISO 14001; industrial safety is certified to OHSAS 18001.
Material recycling
2.8 Product processing/Installation
The metallurgical materials and glass contained in the product
The product system is installed by specially­trained assembly
are suitable for material recycling.
teams.
3 Environmental­Product Declaration ­ dormakaba ­ ST PRO Green
towards energy recovery.
Energy recovery
• EWC 15 01 01 Paper and cardboard packaging
The plastics contained in the product are suitable for energetic
• EWC 15 01 02 Plastic packaging
recovery.
End of Life:
All materials contained in the product are directed to energy
Landfilling
recovery or recycling process.
Is not applicable.
• EWC 16 02 14 Used devices with the exception of those
2.15 Disposal included in 16 02 09 to 16 02 1
Cuttings: • EWC 16 02 16 Components removed from used
Cuttings incurred during the manufacturing phase are directed devices with the exception of those included in 16 02 15
towards metallurgical recycling and energy recovery. Cuttings • EWC 17 02 03 Plastic
are collected separately and collected by a disposal company. • EWC 17 04 02 Aluminum
• EWC 17 04 05 Iron and steel
Following European Waste Catalogue (EWC) Codes are • EWC 17 04 11 Cables with the exception of those
relevant: included in 17 04 10
• EWC 17 02 02 Glass
• EWC 07 02 03 Plastic waste
• EWC 12 01 01 Ferrous metal filings and turnings 2.16 Further information
Contact data for more detailed information:
• EWC 12 01 03 Non­ferrous metal filings and turnings
Please refer to the last page of this Declaration
Packaging:
Packaging incurred for installation in the building is directed
3. LCA: Calculation rules
Recycling of glass and metal scrap results in credits of the
3.1 Declared Unit respective raw materials.
The declared unit is one (1) piece ST PRO Green. The
declared unit consists of the drive system and two sliding 3.3 Estimates and assumptions
panels. The LCA results of two side screens and a fanlight are It was assumed that End­of­Life thermal waste incineration
presented in the appendix. plants are plants with an R1 factor (energy conversion
efficiency or energy efficiency of waste incineration plants
Declared unit
according to the European Waste Framework Directive) >0.6.
Name Value Unit
Declared unit for automatic doors and gates 4.07 m2 3.4 Cut-off criteria
Grammage 50.32 kg/m2 The effect associated with the neglected mass shares is less
than 5% of the effect categories per module. The minimum limit
Mass (total system) 204.83 kg
of 1% total mass and the use of renewable and non­renewable
Conversion factor to 1 kg 0.005 ­ primary energy is not exceeded.
3.2 System boundary 3.5 Background data
Type of the EPD: cradle to gate ­ with options Modules A1-A3, The LCA software GaBi 10.0 was used to model the life cycle.
A4, and A5 The entire manufacturing process, as well as energy
The product stage (A1­A3) begins with considering the consumption, were modelled on the basis of manufacturer­
production of the necessary raw materials and energies, specific data.
including all corresponding upstream chains and the actual However, generic background datasets were used for the
procurement transports. Furthermore, the entire manufacturing upstream and downstream processes. The majority of the
phase was mapped, including the treatment of production background datasets used were taken from the current version
waste until the end­of­waste status (EoW) was reached. In of the GaBi 10.0 database. Ecoinvent Version 3.6 and
addition, both the distribution transports (A4) and the Ecoinvent Version 2.2 datasets were only used when suitable
installation including power­consuming tools, installation GaBi 10.0 datasets were not available.
materials and the packaging waste generated during
installation (A5) were taken into account. Where possible, German datasets were used for modules A1­
A3, and the corresponding European datasets for distribution
Module B6 transports (A4), installation (A5) and disposal scenarios (C
Module B6 includes the operational energy use over the modules).
Reference Service Life of 15 years.
3.6 Data quality
The background datasets used for accounting purposes mainly
Modules C1-C4
originate from the respective updated GaBi 10.0 databases at
The modules include the environmental impacts for dismantling
the time of calculation.
of the ST PRO Green and the treatment of the waste categories
The data for the examined products was captured on the basis
until end­of­waste status (EoW) is reached, including the
of evaluations of internal production and environmental data,
associated transports at the end of the product life cycle.
the collection of LCA­­relevant data within the supply chain, as
well as the evaluation of relevant data for the energy supply.
Module D
The collected data were checked for plausibility and
Identification of the benefits and costs of the product outside
consistency. Good representativity can be assumed.
the system boundary. For plastics, these consist of energy
credits from thermal utilization (C3) in the form of the average
3.7 Period under review
European electricity mix or thermal energy from natural gas.
4 Environmental­Product Declaration ­ dormakaba ­ ST PRO Green
Life cycle assessment data were collected in 2019 and 2020. incinerated at the end of life in a waste incineration plant.
Metallurgical parts and glass are recycled. Any emissions that
3.8 Geographic Representativeness occur are taken into account in the model. Depending on their
Land or region, in which the declared product system is elementary composition and the resulting heating values,
manufactured, used or handled at the end of the product´s recycling credits are taken into account in module D.
lifespan: Germany
3.10 Comparability
Basically, a comparison or an evaluation of EPD data is only
3.9 Allocation
possible if all the data sets to be compared were created
All required energies, raw materials, and supplies could be according to EN 15804 and the building context, respectively
(clearly) assigned to the declared product. No by­­products are the product­specific characteristics of performance, are taken
produced and no allocation is required. In module A1­­A3, into account.
credits are issued for recycling of metallurgical waste.
Packaging materials and the combustible product parts are
4. LCA: Scenarios and additional technical information
Transport to the building site (A4)
Name Value Unit
End of life (C1-C4)
Litres of fuel unknownl/100km
Name Value Unit
Transport distance (Truck) 596 km
Collected separately waste type waste type 204.97 kg
Capacity utilisation (including empty runs)
(Truck) 55 % Collected as mixed construction waste ­ kg
Gross density of products transported unknown kg/m3 Reuse ­ kg
Recycling 192.78 kg
Capacity utilisation volume factor unknown ­
Energy recovery 12.2 kg
Installation into the building (A5) Landfilling ­ kg
Name Value Unit
Reuse, recovery and/or recycling potentials (D), relevant
Auxiliary (screws and screw anchors) 0.155 kg
scenario information
Electricity consumption 0.04 kWh
Name Value Unit
Net steel scrap 8.39 kg
Reference service life Net aluminium scrap 6.65 kg
Name Value Unit Net zinc scrap 0.85 kg
Life Span according to the manufacturer 15 a Collection rate 100 %
Recycling loss 0 %
Operational energy use (B6) and Operational water use
(B7)
Name Value Unit
Electricity consumption (15 years) 988.49 kWh
5 Environmental­Product Declaration ­ dormakaba ­ ST PRO Green
5. LCA: Results
The following table shows the results of the LCA for 1 piece declared ST PRO Green. The results in module B6 are based on a lifetime
of 15 years. The LCA results for two side screens and a fanlight are presented in the appendix.
DESCRIPTION OF THE SYSTEM BOUNDARY (X = INCLUDED IN LCA; MND = MODULE NOT DECLARED; MNR = MODULE NOT
RELEVANT)
BENEFITS
AND LOADS
CONSTRUCTION
BEYOND
PRODUCT STAGE PROCESS USE STAGE END OF LIFE STAGE
THE SYSTEM
STAGE
BOUNDARIE
S
la ire ta m w a Ry lp p u s tro p s n a rT g n iru tc a fu n a M e h t m o rf tro p s n a rTe tis e h t o t e ta g y lb m e s s A e s U e c n a n e tn ia M ria p e R tn e m e c a lp e R tn e m h s ib ru fe R y g re n e la n o ita re p Oe s u re ta w la n o ita re p Oe s u n o itc u rts n o c ­e Dn o itilo m e d tro p s n a rT g n is s e c o rp e ts a W la s o p s iD ­e s u e R­y re v o c e R­g n ilc y c e Rla itn e to p
A1 A2 A3 A4 A5 B1 B2 B3 B4 B5 B6 B7 C1 C2 C3 C4 D
X X X X X MND MND MNR MNR MNR X MND X X X X X
RESULTS OF THE LCA - ENVIRONMENTAL IMPACT according to EN 15804+A1: 1 piece ST PRO Green
Parameter Unit A1-A3 A4 A5 B6 C1 C2 C3 C4 D
GWP kg CO 2 eq 5.9E+02 1.02E+01 4.99E+00 3.9E+02 8.22E­03 4.91E­01 3.23E+01 0 ­1.04E+02
ODP kg CFC11 eq 1.13E­05 1.68E­15 5.95E­15 1.17E­11 2.46E­16 1.43E­16 1.63E­07 0 ­4.83E­08
AP kg SO 2 eq 4.22E+00 4.32E­02 2.23E­03 8.19E­01 1.73E­05 2.09E­03 3.17E­02 0 ­4.48E­01
EP kg PO 43 eq 8.97E­01 1.08E­02 3.36E­04 9.06E­02 1.91E­06 5.23E­04 1.74E­02 0 ­5.19E­02
POCP kg Ethen eq 2.53E­01 ­1.82E­02 2.01E­04 5.83E­02 1.23E­06 ­7.85E­04 1.69E­03 0 ­3.18E­02
ADPE kg Sb eq 6.13E­02 8.51E­07 2.35E­05 1.3E­04 2.75E­09 4.6E­08 7.47E­05 0 ­3.73E­03
ADPF MJ 8.42E+03 1.4E+02 9.73E+00 4.32E+03 9.11E­02 6.71E+00 5.24E+01 0 ­1.19E+03
GWP = Global warming potential; ODP = Depletion potential of the stratospheric ozone layer; AP = Acidification potential of land and water; EP =
Eutrophication potential; POCP = Formation potential of tropospheric ozone photochemical oxidants; ADPE = Abiotic depletion potential for non­fossil
resources; ADPF = Abiotic depletion potential for fossil resources
RESULTS OF THE LCA - INDICATORS TO DESCRIBE RESOURCE USE according to EN 15804+A1: 1 piece ST PRO Green
Parameter Unit A1-A3 A4 A5 B6 C1 C2 C3 C4 D
PERE MJ 1.18E+03 7.86E+00 3.91E+01 3.1E+03 6.53E­02 3.91E­01 1.4E+01 0 ­3.47E+02
PERM MJ 3.98E+01 0 ­3.77E+01 0 0 0 ­2.06E+00 0 0
PERT MJ 1.22E+03 7.86E+00 1.36E+00 3.1E+03 6.53E­02 3.91E­01 1.19E+01 0 ­3.47E+02
PENRE MJ 8.96E+03 1.4E+02 1.08E+01 7E+03 1.47E­01 6.74E+00 5.15E+02 0 ­1.34E+03
PENRM MJ 4.56E+02 0 ­3.44E­01 0 0 0 ­4.56E+02 0 0
PENRT MJ 9.42E+03 1.4E+02 1.05E+01 7E+03 1.47E­01 6.74E+00 5.89E+01 0 ­1.34E+03
SM kg 4.07E+01 0 0 0 0 0 0 0 1.55E+02
RSF MJ 0 0 0 0 0 0 0 0 0
NRSF MJ 0 0 0 0 0 0 0 0 0
FW m3 8.39E+00 9.1E­03 1.41E­02 3.59E+00 7.56E­05 4.34E­04 8.88E­02 0 ­4.02E+00
PERE = Use of renewable primary energy excluding renewable primary energy resources used as raw materials; PERM = Use of renewable primary
energy resources used as raw materials; PERT = Total use of renewable primary energy resources; PENRE = Use of non­renewable primary energy
excluding non­renewable primary energy resources used as raw materials; PENRM = Use of non­renewable primary energy resources used as raw
materials; PENRT = Total use of non­renewable primary energy resources; SM = Use of secondary material; RSF = Use of renewable secondary fuels;
NRSF = Use of non­renewable secondary fuels; FW = Use of net fresh water
RESULTS OF THE LCA – WASTE CATEGORIES AND OUTPUT FLOWS according to EN 15804+A1:
1 piece ST PRO Green
Parameter Unit A1-A3 A4 A5 B6 C1 C2 C3 C4 D
HWD kg 1.57E­02 6.52E­06 2.41E­08 2.9E­06 6.1E­11 3E­07 1.91E­07 0 ­2.68E­06
NHWD kg 1.81E+02 2.14E­02 1.39E­01 4.96E+00 1.05E­04 1.09E­03 1.17E+01 0 ­1.66E+01
RWD kg 3.08E­01 1.73E­04 3.15E­04 1.06E+00 2.24E­05 1.18E­05 1.57E­03 0 ­5.88E­02
CRU kg 0 0 0 0 0 0 0 0 0
MFR kg 8.87E+00 0 0 0 0 0 1.93E+02 0 0
MER kg 2.66E+00 0 2.98E+00 0 0 0 1.2E+01 0 0
EEE MJ 0 0 6.57E+00 0 0 0 3.82E+01 0 0
EET MJ 0 0 1.19E+01 0 0 0 2.81E+02 0 0
HWD = Hazardous waste disposed; NHWD = Non­hazardous waste disposed; RWD = Radioactive waste disposed; CRU = Components for re­use;
MFR = Materials for recycling; MER = Materials for energy recovery; EEE = Exported electrical energy; EET = Exported thermal energy
6. LCA: Interpretation
6 Environmental­Product Declaration ­ dormakaba ­ ST PRO Green
The CML characterization factors were used for the evaluation. (>90%). Acidification potential (AP) in modules A1­A3 is
The results of the CML categories refer to the potential dominated by the glass (48%) and the operator (27%).
environmental impacts over a period of 100 years. Eutrophication potential (EP) in modules A1­A3 is dominated by
The main impacts lie in the modules A1­A3 and B6. The the operator (71%) and there the electronic components. The
impacts in module B6 are due to the electricity mix used for glass also has a significant impact on the EP (23%).
modelling the electricity consumption over a period of 15 years. Formation potential of tropospheric ozone photochemical
In the following, the main influences on the modules A1­A3 for oxidants (POCP) in modules A1­A3 is mainly influenced by the
the indicators will be explained. glass.
Abiotic depletion potential for non­­fossil resources in modules
Global warming potential (GWP) in modules A1­A3 is mainly A1­A3 is dominated by the operator (91%) and there the
influenced by the operator (35%), the glass (35%) and electronic components.
aluminium (20%). Ozone depletion potential in module A1­A3 is Abiotic depletion potential for fossil resources (ADPF) in
mainly influenced by the electronic components of the operator modules A1­A3 is dominated by the glass (47%).
7. Requisite evidence
8. References
Standards Limits ­ Limits for harmonic current emissions (equipment input
current ≤ 16 A per phase).
EN 15804 EN 61000-3-3
EN 15804:2012­04+A1 2013, Sustainability of construction DIN EN 61000­3­3:2014­03, Electromagnetic compatibility
works — Environmental Product Declarations — Core rules for (EMC) ­ Part 3­3:
the product category of construction products. Limits ­ Limitation of voltage changes, voltage fluctuations and
EN 16005 flicker in public low­voltage supply systems, for equipment with
rated current ≤ 16 A per phase and not subject to conditional
DIN EN 16005:2013­01 and Amendment 2015­10, Power connection.
operated pedestrian doorsets ­ Safety in use ­ Requirements EN 61000-6-2
and test methods.
EN 60335-2-103 DIN EN 61000­6­2:2005 + Amendment:2011. Electromagnetic
compatibility (EMC) ­ Part 6­2: Generic standards ­ Immunity
DIN EN 60335­2­103:2016­05, Household and similar electrical standard for industrial environments.
appliances ­ Safety ­ Part 2­103: Particular requirements for EN 61000-6-3
drives for gates, doors and windows.
EN 61000-3-2 DIN EN 61000­6­3:2007 + A1:2011, Electromagnetic
compatibility (EMC) ­ Part 6­3: Generic standards ­ Emission
DIN EN 61000­3­2:2015­03, Electromagnetic compatibility standard for residential, commercial and light­industrial
(EMC) ­ Part 3­2: environments.
7 Environmental­Product Declaration ­ dormakaba ­ ST PRO Green
IEC 63000 Database for life cycle assessment (life cycle inventory data),
Version 2.2, 2010.
DIN EN IEC 63000:2019­05, Technical documentation for the
assessment of electrical and electronic products with respect to Ecoinvent Version 3.6
the restriction of hazardous substances. Database for life cycle assessment (life cycle inventory data),
ISO 9001 Version 3.6, 2019.
DIN EN ISO 9001:2015­11, Quality management systems ­ EWC
Requirements (ISO 9001:2015); German and English version European Waste Catalogue (EWC). Commission Decision on
EN ISO 9001:2015 ISO 12100 the European List of Waste (COM 2000/532/EC)
DIN EN ISO 12100:2011­03, Safety of machinery ­ General GaBi 10.0
principles for design ­ Risk assessment and risk reduction. Life cycle engineering (GaBi) software and database. LBP,
ISO 13849-1 University of Stuttgart and thinkstep AG, Documentation of
GaBi 10.0 data sets http://documentation.gabisoftware.com/,
DIN EN ISO 13849­1:2016­06, Safety of machinery ­ Safety­ 2020.
related parts of control systems ­ Part 1: General principles for
design. IBU 2016
ISO 14001 Institut Bauen und Umwelt e.V.: General Programme
Instructions for the Preparation of EPDs at the Institut Bauen
ISO 14001:2015­09, Environmental management systems ­ und Umwelt e.V. Version 1., Berlin: Institut Bauen und Umwelt
Requirements with guidance for use ISO 14025 e.V., 2016. www.ibu­epd.com
DIN EN ISO 14025:2011­10, Environmental labels and IP
declarations — Type III environmental declarations — Ingress Protection Rating. DIN EN 60529; VDE 04701: 201409:
Principles and procedures. Degrees of protection provided by enclosures (IP Code) (IEC
OHSAS 18001 60529:1989 + A1:1999 + A2:2013); German version EN
60529:1991 + A1:2000 + A2:2013
Occupational health and safety – Management systems –
Requirements Machinery Directive 2006/42/EC
Further references Directive 2006/42/EC of the European Parliament and of the
Council of 17 May 2006 on machinery, and amending Directive
2011/65/EU ROHS3 Directive 95/16/EC (recast)
Directive 2011/65/EU of the European Parliament and of the
Council of 8 June 2011 on the restriction of the use of certain Ordinance on Biocide Products No. 528/2012
hazardous substances in electrical and electronic equipment Regulation (EU) No 528/2012 of the European Parliament and
of the Council of 22 May 2012 concerning the making available
2014/30/EU Electromagnetic Compatibility Directive on the market and use of biocidal products
Directive 2014/30/EU of the European Parliament and of the
Council of 26 February 2014 on the harmonisation of the laws Product Category Rules Part A
of the Member States relating to electromagnetic compatibility Calculation Rules for the Life Cycle Assessment and
(recast) Requirements on the Project Report. Version 1.8 (04.07.2019)
CML Product Category Rules Part B
Institute of Environmental Sciences Leiden University Requirements on the EPD for Automatic doors, automatic
gates, and revolving door systems. Version 1.1 (09.07.2013)
Ecoinvent Version 2.2
8 Environmental­Product Declaration ­ dormakaba ­ ST PRO Green
Publisher
Institut Bauen und Umwelt e.V. +49 (0)30 3087748­ 0
Hegelplatz 1 info@ibu­epd.com
10117 Berlin www.ibu­epd.com
Germany
Programme holder
Institut Bauen und Umwelt e.V. +49 (0)30 3087748­ 0
Hegelplatz 1 info@ibu­epd.com
10117 Berlin www.ibu­epd.com
Germany
Author of the Life Cycle Assessment
brands & values GmbH +49 421 70 90 84 33
Altenwall 14 info@brandsandvalues.com
28195 Bremen www.brandsandvalues.com
Germany
Owner of the Declaration
dormakaba International Holding GmbH +49 2333 793­0
DORMA Platz 1 info.de@dormakaba.com
58256 Ennepetal www.dormakaba.com
Germany
9 Environmental­Product Declaration ­ dormakaba ­ ST PRO Green
