ENVIRONMENTAL PRODUCT DECLARATION
as per ISO 14025 and EN 15804+A2
Owner of the Declaration European Association for Panels and Profiles e. V. (PPA-Europe)
Publisher Institut Bauen und Umwelt e.V. (IBU)
Programme holder Institut Bauen und Umwelt e.V. (IBU)
Declaration number EPD-PPA-20240129-CBG2-EN
Issue date 19.07.2024
Valid to 18.07.2029
Profiled sheets made of steel for roof, wall, deck and ceiling
constructions
PPA-Europe
www.ibu-epd.com | https://epd-online.com
General Information
PPA-Europe Profiled sheets made of steel for roof, wall, deck
and ceiling constructions
Programme holder Owner of the declaration
IBU – Institut Bauen und Umwelt e.V. European Association for Panels and Profiles e. V. (PPA-Europe)
Hegelplatz 1 Europark Fichtenhain A 13a
10117 Berlin 47807 Krefeld
Germany Germany
Declaration number Declared product / declared unit
EPD-PPA-20240129-CBG2-EN 1m² industrially produced steel profiled sheets
This declaration is based on the product category rules: Scope:
Thin walled profiles and profiled panels of metal, 01.08.2021 This document is an association EPD for 1 m² of steel trapezoidal 135/310
(PCR checked and approved by the SVR) profile and it represents an average EPD, based on vertical averaging of
the specific producer datasets under consideration of the yearly production
amounts. Its applicability is limited to steel profiled sheets, which are
Issue date manufactured by member companies of the European Association for
Panels and Profiles.
19.07.2024
The following member companies of the European Association for Panels
and Profiles have provided data for the year 2022:
Valid to
18.07.2029 1. ArcelorMittal Group, Construction Division
• ArcelorMittal Construction Austria
• ArcelorMittal Construction Belgium
• ArcelorMittal Construction Deutschland
• ArcelorMittal Construcción España
• ArcelorMittal Construction France
• ArcelorMittal Construction Nederland
• Arcelormittal Construction Polska
• ArcelorMittal Construção Portugal
• ArcelorMittal Construction Slovakia
• ArcelorMittal Construction Sverige
• Europerfil
Dipl.-Ing. Hans Peters • Münker Metallprofile
(Chairman of Institut Bauen und Umwelt e.V.) 2. Fischer Profil
3. Hans Laukien
4. Isolpack
5. Joris Ide Belgium
6. MAAS Profilzentrum
7. Montana Bausysteme
8. PAGOUNI
9. SAB-profiel
10. Wurzer Profiliertechnik
11. Zambelli RIB-ROOF
These companies are representative for the European production of steel
profiled sheets.
Additionally, the EPD includes a public annex. This annex applies to:
• 1 m² steel trapezoidal profile 35/207
• 1 m² steel standing seam profile
• 1 m² steel liner tray
• 1 kg steel profile.
The owner of the declaration shall be liable for the underlying information
and evidence; the IBU shall not be liable with respect to manufacturer
information, life cycle assessment data and evidences.
The EPD was created according to the specifications of EN 15804+A2. In
the following, the standard will be simplified as EN 15804.
Verification
The standard EN 15804 serves as the core PCR
Independent verification of the declaration and data according to ISO
14025:2011
internally X externally
1 Environmental Product Declaration - PPA-Europe - Profiled sheets made of steel for roof, wall, deck and ceiling constructions
Florian Pronold Mr Olivier Muller,
(Managing Director Institut Bauen und Umwelt e.V.) (Independent verifier)
2 Environmental Product Declaration - PPA-Europe - Profiled sheets made of steel for roof, wall, deck and ceiling constructions
Product
Performance data of the product in accordance with the
Product description/Product definition declaration of performance with respect to its essential
The EPD is valid for prefabricated thin-walled profiled sheets characteristics according to EN 14782 or EN 1090.
made of steel for load-bearing, self-supporting and non-
supporting applications in single- and multi-layer roof, wall, Base materials/Ancillary materials
deck and ceiling structures. Steel sheet according to EN 10346:
S280 GD to S350 GD
The profiled sheets are made of a core of steel, which is
protected against corrosion with zinc and organic coatings. The Metallic coating according to EN 10346:
LCA is based on vertical averaging of the specific producer Zinc Z275, coating 275 g/m²
datasets under consideration of the respective yearly
production amounts. The zinc layer has a content of at least 99 weight percent zinc
and typical thickness of 20 μm.
For the placing of the product on the market in the European
Union / European Free Trade Association (EU/EFTA) (with the Organic coating according to EN 10169:
exception of Switzerland), CPR applies. The product needs a Polyester (SP), coil coating, 25 μm on the application side and
Declaration of Performance taking into consideration EN 14782 max. 15 μm on the backside.
or EN 1090 and the CE-marking. The data listed in the
respective Declaration of Performance apply. The product does not contain any SVHCs (Substances of Very
High Concern) REACH.
For the application and use, the respective national provisions
apply. Reference service life
Thin-walled profiled sheets made of steel used in lightweight
Application metal constructions must withstand a term of protection of at
The products are used as covering components in single- and least 15 years. The term of protection is the period until first
multi-layer roof and wall structures, as well as supporting trays slight renewals in the surface are required, only if there is no
in single- and multi-layer roof, wall, deck and ceiling structures need of frequent inspections and service.
for mainly static loads.
The term of protection depends on the location, weather
The profiled sheets are used in interior and exterior conditions and the quality of the coating.
applications.
The reference service life for the product range of steel profiled
Technical Data sheets is not declared, since the lifetime will depend on specific
Technical specifications for profiled sheets are: applications as well as environmental conditions. As a structural
• EN 14782 part of the building, steel profiled sheets are expected and
• EN 508 specified to reach the same service life as that of the building.
• EN 1090 The steel reference service life can be of > 50 years.
Constructional data
The information in this section does not refer to a reference
Trapezoidal profile 135/310 service life according to ISO 15686.
Name Value Unit
Thickness of the sheet, according EN 10143 0.75 mm
Surface weight 8.87 kg/m²
Height of the profile, according EN 508 or EN 135 -
mm
1090 137
LCA: Calculation rules
provide materials and energy input for the system,
Declared Unit manufacturing and transport processes up to the factory gate,
The declared unit is 1 m2 of steel profile. The averaging is done as well as waste processing.
weighted based on the production volume (in m²) per company. Module A4: Delivery to the construction site- fixed transport
distance of 100 km.
Declared unit
Module A5: Disposal of transport packaging at the construction
Name Value Unit
site and installation by construction machineries- diesel and
Declared unit 1 m2 electricity driven.
Grammage (surface weight) 8.87 kg/m2
Module C1: Dismantling with the use of machineries- diesel and
Conversion factor to 1 kg 0.113 -
electricity driven.
Layer thickness (coating outside) 2.5e-5 m
Module C2: Transport to the site of end-of-life treatment- fixed
transport distance of 50 km.
System boundary
Module C3: Metal recycling of the steel profiles
Type of the EPD: cradle to gate - with options, modules C1-C4 Module C4: Deposition/landfill (no environmental impact).
and module D (A1-A3, C, D and additional modules A4 and A5)
Module D: Potential credits for substitution processes or
Production stage (modules A1-A3) includes processes that recycling materials from A5 and C3. For the end of life, it is
3 Environmental Product Declaration - PPA-Europe - Profiled sheets made of steel for roof, wall, deck and ceiling constructions
assumed that the steel is recycled with credit for the recycling
potential declared in module D. Comparability
For the end of life, a collection rate of 100 % is assumed. Basically, a comparison or an evaluation of EPD data is only
possible if all the data sets to be compared were created
Geographic Representativeness according to EN 15804 and the building context, respectively
Land or region, in which the declared product system is the product-specific characteristics of performance, are taken
manufactured, used or handled at the end of the product´s into account. LCA FE (fka GaBi) software and database CUP
lifespan: Europe 2023.1 LCA FE were used as calculation basis.
LCA: Scenarios and additional technical information
Packaging materials:
Characteristic product properties of biogenic carbon PE film 0.010 kg/m² profile
Information on describing the biogenic Carbon Content at Wooden pallets 0.140 kg/m² profile
factory gate A5 covers the waste treatment of packaging material at the
point of installation.
Name ValueUnit
Name ValueUnit
kg
Biogenic carbon content in product - C Output substances following waste treatment on 0.15 kg
site
Biogenic carbon content in accompanying kg
packaging 0.05 C Machines for installation - diesel driven, per kg 0.004 L
Machines for installation - electricity driven, per kg 1.89 Wh
Note: 1 kg of biogenic carbon is equivalent to 44/12 kg of CO
2
End of life (C1-C4)
Note: 1 kg of biogenic carbon is equivalent to 44/12 kg of CO .
2 Name ValueUnit
Machines for dismantling - diesel driven, per kg 0.005 L
Machines for dismantling - electricity driven, per kg 0.63 Wh
The following technical information is a basis for the declared
modules. Collected separately waste type 8.87 kg
Recycling 8.87 kg
Transport to the building site (A4)
Landfilling - kg
Name Value Unit
Transport distance 100 km Reuse, recovery or recycling potential (D)
Capacity utilisation (including empty runs) 61 %
The avoided production of primary steel sheet is considered.
Installation into the building (A5) Resulting potential benefits and loads for the metal recycling
are declared in module D.
4 Environmental Product Declaration - PPA-Europe - Profiled sheets made of steel for roof, wall, deck and ceiling constructions
LCA: Results
DESCRIPTION OF THE SYSTEM BOUNDARY (X = INCLUDED IN LCA; MND = MODULE OR INDICATOR NOT DECLARED; MNR
= MODULE NOT RELEVANT)
Benefits and
Construction loads beyond
Product stage Use stage End of life stage
process stage the system
boundaries
la ire ta m w a Ry lp p u s tro p s n a rT g n iru tc a fu n a M e h t m o rf tro p s n a rTe tis e h t o t e ta g y lb m e s s A e s U e c n a n e tn ia M ria p e R tn e m e c a lp e R tn e m h s ib ru fe R y g re n e la n o ita re p Oe s u re ta w la n o ita re p Oe s u n o itc u rts n o c -e Dn o itilo m e d tro p s n a rT g n is s e c o rp e ts a W la s o p s iD -e s u e R-y re v o c e R-g n ilc y c e Rla itn e to p
A1 A2 A3 A4 A5 B1 B2 B3 B4 B5 B6 B7 C1 C2 C3 C4 D
X X X X X MND MND MNR MNR MNR MND MND X X X X X
RESULTS OF THE LCA - ENVIRONMENTAL IMPACT according to EN 15804+A2: 1 m² steel trapezoidal profile 135/310 (8.87
kg/m²)
Parameter Unit A1-A3 A4 A5 C1 C2 C3 C4 D
GWP-total kg CO 2 eq 2.6E+01 6.43E-02 5.84E-01 4.11E-01 3.21E-02 0 0 -1.79E+01
GWP-fossil kg CO 2 eq 2.62E+01 6.35E-02 3.67E-01 4.05E-01 3.18E-02 0 0 -1.79E+01
GWP-biogenic kg CO 2 eq -1.93E-01 1.88E-04 2.13E-01 1.61E-03 9.38E-05 0 0 3.47E-02
GWP-luluc kg CO 2 eq 1.02E-02 5.88E-04 3.16E-03 3.73E-03 2.94E-04 0 0 -7.39E-03
ODP kg CFC11 eq 2.22E-11 8.27E-15 1.64E-11 8.17E-14 4.13E-15 0 0 5.19E-11
AP mol H+ eq 6.29E-02 8.15E-05 2.05E-03 2.37E-03 4.08E-05 0 0 -4.02E-02
EP-freshwater kg P eq 2.16E-05 2.32E-07 1.27E-06 1.48E-06 1.16E-07 0 0 -1.36E-06
EP-marine kg N eq 1.54E-02 2.76E-05 9.9E-04 1.15E-03 1.38E-05 0 0 -9.65E-03
EP-terrestrial mol N eq 1.66E-01 3.33E-04 1.1E-02 1.28E-02 1.66E-04 0 0 -1.04E-01
kg NMVOC
POCP 4.92E-02 7.03E-05 2.63E-03 3.07E-03 3.51E-05 0 0 -3.21E-02
eq
ADPE kg Sb eq 6.55E-04 4.18E-09 2.34E-08 2.68E-08 2.09E-09 0 0 -1.87E-07
ADPF MJ 2.5E+02 8.66E-01 4.8E+00 5.52E+00 4.33E-01 0 0 -1.33E+02
m3 world eq
WDP 8.43E-01 7.68E-04 3.07E-02 5.22E-03 3.84E-04 0 0 -2.57E-01
deprived
GWP = Global warming potential; ODP = Depletion potential of the stratospheric ozone layer; AP = Acidification potential of land and water; EP =
Eutrophication potential; POCP = Formation potential of tropospheric ozone photochemical oxidants; ADPE = Abiotic depletion potential for non-fossil
resources; ADPF = Abiotic depletion potential for fossil resources; WDP = Water (user) deprivation potential)
RESULTS OF THE LCA - INDICATORS TO DESCRIBE RESOURCE USE according to EN 15804+A2: 1 m² steel trapezoidal
profile 135/310 (8.87 kg/m²)
Parameter Unit A1-A3 A4 A5 C1 C2 C3 C4 D
PERE MJ 2.12E+01 6.3E-02 2.96E+00 4.19E-01 3.15E-02 0 0 2.18E+01
PERM MJ 2.55E+00 0 -2.55E+00 0 0 0 0 0
PERT MJ 2.37E+01 6.3E-02 4.11E-01 4.19E-01 3.15E-02 0 0 2.18E+01
PENRE MJ 2.51E+02 8.69E-01 5.43E+00 5.54E+00 4.34E-01 0 0 -1.35E+02
PENRM MJ 6.04E-01 0 -6.04E-01 0 0 0 0 0
PENRT MJ 2.52E+02 8.69E-01 4.82E+00 5.54E+00 4.34E-01 0 0 -1.35E+02
SM kg 2.14E+00 0 0 0 0 0 0 0
RSF MJ 3.84E-22 0 0 0 0 0 0 0
NRSF MJ 4.51E-21 0 0 0 0 0 0 0
FW m3 3.13E-02 6.9E-05 1.02E-03 4.54E-04 3.45E-05 0 0 -1.16E-02
PERE = Use of renewable primary energy excluding renewable primary energy resources used as raw materials; PERM = Use of renewable primary
energy resources used as raw materials; PERT = Total use of renewable primary energy resources; PENRE = Use of non-renewable primary energy
excluding non-renewable primary energy resources used as raw materials; PENRM = Use of non-renewable primary energy resources used as raw
materials; PENRT = Total use of non-renewable primary energy resources; SM = Use of secondary material; RSF = Use of renewable secondary fuels;
NRSF = Use of non-renewable secondary fuels; FW = Use of net fresh water
RESULTS OF THE LCA – WASTE CATEGORIES AND OUTPUT FLOWS according to EN 15804+A2:
1 m² steel trapezoidal profile 135/310 (8.87 kg/m²)
Parameter Unit A1-A3 A4 A5 C1 C2 C3 C4 D
HWD kg 8.35E-06 2.69E-12 7.81E-12 1.44E-11 1.35E-12 0 0 -5.09E-10
NHWD kg 1.34E+00 1.32E-04 5.03E-03 8.64E-04 6.62E-05 0 0 -2.65E-01
RWD kg 3.21E-03 1.63E-06 2.8E-05 1.56E-05 8.13E-07 0 0 2.21E-03
CRU kg 0 0 0 0 0 0 0 0
MFR kg 1.65E-01 0 0 0 0 8.87E+00 0 0
MER kg 0 0 0 0 0 0 0 0
EEE MJ 0 0 0 0 0 0 0 0
5 Environmental Product Declaration - PPA-Europe - Profiled sheets made of steel for roof, wall, deck and ceiling constructions
EET MJ 0 0 0 0 0 0 0 0
HWD = Hazardous waste disposed; NHWD = Non-hazardous waste disposed; RWD = Radioactive waste disposed; CRU = Components for re-use;
MFR = Materials for recycling; MER = Materials for energy recovery; EEE = Exported electrical energy; EET = Exported thermal energy
RESULTS OF THE LCA – additional impact categories according to EN 15804+A2-optional:
1 m² steel trapezoidal profile 135/310 (8.87 kg/m²)
Parameter Unit A1-A3 A4 A5 C1 C2 C3 C4 D
Disease
PM 9.07E-07 5.97E-10 4.02E-08 4.71E-08 2.98E-10 0 0 -5.87E-07
incidence
IR kBq U235 eq 3.5E-01 2.42E-04 4.45E-03 2.42E-03 1.21E-04 0 0 2.39E-01
ETP-fw CTUe 5.04E+01 6.15E-01 3.37E+00 3.91E+00 3.07E-01 0 0 -2.31E+01
HTP-c CTUh 3.07E-08 1.26E-11 7.13E-11 8.02E-11 6.29E-12 0 0 -2.74E-08
HTP-nc CTUh 3.32E-07 6.7E-10 4.64E-09 5.26E-09 3.35E-10 0 0 -1.07E-07
SQP SQP 5.31E+01 3.62E-01 2E+00 2.31E+00 1.81E-01 0 0 1.23E+01
PM = Potential incidence of disease due to PM emissions; IR = Potential Human exposure efficiency relative to U235; ETP-fw = Potential comparative
Toxic Unit for ecosystems; HTP-c = Potential comparative Toxic Unit for humans (cancerogenic); HTP-nc = Potential comparative Toxic Unit for humans
(not cancerogenic); SQP = Potential soil quality index
Disclaimer 1 – concerning Potential Human exposure efficiency relative
to U235 (IRP) - This impact category deals mainly with the eventual impact of low-dose ionizing radiation on human health of the
nuclear fuel cycle. It does not consider effects due to possible nuclear accidents, occupational exposure or radioactive waste disposal
in underground facilities. Potential ionizing radiation from the soil, radon and from some construction materials is also not measured by
this indicator.
Disclaimer 2 – concerning (ADP-minerals & metals,
ADP-fossil, WDP, ETP-fwm HTP-c, HTP-nc, SQP) - The results of this environmental impact indicator shall be used with care as the
uncertainties on these results are high as there is limited experience with the indicator.
References
EN 508-1 LCA FE Software and Database
Roofing and cladding products from metal sheet - Specification LCA FE software-system and CUP 2023.1 databases,
for self-supporting products of steel, aluminium or stainless University of Stuttgart and Sphera Solutions GmbH, Leinfelden-
steel sheet - Part 1: Steel Echterdingen, 2023 https://sphera.com/product-
sustainabilitygabi-data-search/
EN 1090-1
Execution of steel structures and aluminium structures - Part 1:
Requirements for conformity assessment of structural
components
EN 1090-4
Execution of steel structures and aluminium structures - Part 4:
Technical requirements for thin-gauge, cold-formed steel
elements and structures for roof, ceiling, floor and wall
applications
EN 14782
Self-supporting metal sheet for roofing, external cladding and
internal lining - Product specification and requirements
EN 15804+ A2:2019
Sustainability of construction works -Environmental Product
Declarations - Core rules for the product category of
construction products
CPR
REGULATION (EU) No 305/2011 OF THE EUROPEAN
PARLIAMENT AND OF THE COUNCIL of 9 March 2011 laying
down harmonised conditions for the marketing of construction
products and repealing Council Directive 89/106/EEC
IBU PCR Part A
PCR - Part A: Calculation rules for the Life Cycle Assessment
and Requirements on the Background Report, version 1.3,
Institut Bauen und Umwelt e.V., www.bau-umwelt.com, August
2021
IBU PCR Part B
PCR – Part B: Requirements of the EPD for thin walled profiles
and profiled panels of metal, v8, Institut Bauen und Umwelt
e.V., www.bau-umwelt.com, 2023-10
6 Environmental Product Declaration - PPA-Europe - Profiled sheets made of steel for roof, wall, deck and ceiling constructions
7 Environmental Product Declaration - PPA-Europe - Profiled sheets made of steel for roof, wall, deck and ceiling constructions
Publisher
Institut Bauen und Umwelt e.V. +49 (0)30 3087748- 0
Hegelplatz 1 info@ibu-epd.com
10117 Berlin www.ibu-epd.com
Germany
Programme holder
Institut Bauen und Umwelt e.V. +49 (0)30 3087748- 0
Hegelplatz 1 info@ibu-epd.com
10117 Berlin www.ibu-epd.com
Germany
Author of the Life Cycle Assessment
Sphera Solutions GmbH +49 (0)711 341817-0
Hauptstraße 111- 113 info@sphera.com
70771 Leinfelden-Echterdingen www.sphera.com
Germany
Owner of the Declaration
European Association for Panels and Profiles e. V. +49 2151 93630-0
(PPA-Europe) info@ppa-europe.eu
Europark Fichtenhain A 13a www.ppa-europe.eu
47807 Krefeld
Germany
8 Environmental Product Declaration - PPA-Europe - Profiled sheets made of steel for roof, wall, deck and ceiling constructions
