Environmental Product Declaration
In accordance with ISO 14025 and EN 15804+A2
Steel piles
Owner of the declaration: Program holder and publisher:
Ferrometall AS The Norwegian EPD foundation
Product name: Declaration number:
Steel piles
NEPD-4793-4044-EN
Declared unit: Registration Number:
1 kg of steel piles
NEPD-4793-4044-EN
Product category /PCR: Issue date:
EN 15804:2012+A2:2019 serves as core PCR.
NPCR 013:2019 Part B for Steel and Aluminium
for Construction Products, version 4.0, issued
2V1a.l0id8 .t2o0:2 3
06.10.2021
The Norwegian
21.08.2028
EPD Foundation
General information
Product: Owner of the declaration:
Steel piles Ferrometall AS
Contact person: Rune Humlebekk
Program Operator: Phone: +47 48 29 04 29
e-mail: rune@ferrometall.no
The Norwegian EPD Foundation
Post Box 5250 Majorstuen, 0303 Oslo, Norway
Tlf: +47 23 08 80 00 Manufacturer:
e-mail: post@epd-norge.no Ferrometall AS
Gyldenløves plass 1, 3044 Drammen
Declaration Number: Phone: +47 32 89 10 30
e-mail: info@ferrometall.no
NEPD-4793-4044-EN Place of production:
This declaration is based on Product
Klaipeda, Lithuania
Category Rules:
EN 15804:2012+A2:2019 serves as core PCR
Management system:
NPCR 013:2019 Part B for Steel and Aluminium
Construction Products. Version 4.0. EN ISO 9001, EN ISO 14001, BS/EN 1090
Statements: Organisation no:
The owner of the declaration shall be liable for the 995 727 064
underlying information and evidence. EPD
Norway shall not be liable with respect to Issue date:
manufacturer, life cycle assessment data and
evidences.
21.08.2023
Valid to:
Declared unit:
1 kg of steel piles
21.08.2028
Year of study:
Declared unit with option:
2023
1 kg of steel piles, cradle-to-gate A1-A3, with
options A4, C1-C4, D
Comparability:
EPDs from other programmes than EPD Norge
Functional unit:
may not be comparable.
-
The EPD has been worked out by:
Verification:
Dan André Johansen, Asplan Viak AS
Independent verification of the declaration and
data, according to ISO14025:2010
internal external ☒
Sign
Ole M. K. Iversen
Approved (Manager of EPD Norway)
Independent verifier approved by EPD Norway
EPD for the best environmental decision 2
Product
Product description:
Threaded steel core piles is a typical construction material for buildings and infrastructure.
Steel core piles are round bars of solid steel that are drilled into the ground, and may be used
alone, or in combination with steel tubes. If used together with steel tubes, the tube casing and
steel core will be rammed into place, and the space between the core and the casings may be
filled with concrete. Steel core piles may be delivered with tapered threads, which are CNC
machined, and the bars are cut at exact lengths according to the intended use. Splicing is done
by threads or welding.
Products start out as pre-produced steel components from round rolled steel produced at
various destinations in Europe. The steel components are drilled/turned for production of
threaded steel core piles for use in piling applications. Products will vary in size and shape and
are produced in accordance with specific project needs.
Product specification:
Materials kg %
Steel with alloys 1,00 100
Technical data:
Standard dimensions: Ø50 mm–300 mm, 6-8-12 meter lengths and steel grades S355J2. DNV-GL
documentation of capacity from Ø70–Ø230 mm. Recycled content in the final product is
calculated to be approximately 37,4%.
Market:
Norway and Scandinavia
Reference service life, product:
60 years
Reference service life, building:
60 years
LCA: Calculation rules
Declared unit:
1 kg of steel piles, cradle-to-gate A1-A3 with options A4, C1-C4 and D.d
Data quality:
General requirements and guidelines concerning the use of generic and specific data and the
quality of those are as described in EN 15804: 2012+A2:2019, clause 6.3.7 and 6.3.8., including
ISO14044:2006, 4.2.3.6. The data is representative according to temporal, geographical and
technological requirements. Generic data is from LCA databases such as ecoinvent v3.8, Agri-
footprint 5 and World Steel Association LCI data which is found in the Industry data 2.0
EPD for the best environmental decision 3
ecoinvent extension (See also Worldsteel, 2017). Calculations have been carried out using
Simapro v9. Characterization factors from EN15804:2012 + A2:2019.
Allocation:
The allocation is made in accordance with the provisions of EN 15804. Production activities,
energy, water and waste production in-house is allocated equally among all products through
mass allocation. Effects of primary production of recycled materials allocated to the main
product in which the material was used. The recycling process and transportation of the
material is allocated to this analysis.
System boundary:
Modules are declared according to NPCR 013 Part B. Declared modules are shown in Figure 1.
Gray boxes denote modules not declared.
Figure 1: System boundaries
Cut-off criteria:
All major raw materials and all the essential energy is included. The production process for raw
materials and energy flows that are included with very small amounts (<1% energy, mass,
impact) are not included. This cut-off rule does not apply for hazardous materials and
substances.
LCA: Scenarios and additional technical information
The following information describe the scenarios in the different modules of the EPD.
Transport from Klaipeda, Lithuania to Horten, Norway, and transport by truck to
the user (A4)
Capacity utilisation (incl. Distance Fuel/Energy value
Type Type of vehicle
return) % km consumption (kg/t)
Ship 80% 5000 DWT 922 0,014 kg/tkm 12,9
Truck 80 % Unspecified, EURO6 47 0,025 kg/tkm 1,2
Truck 80% Lorry>32t, EURO6 300 0,025 kg/tkm 7,5
Scenario for distance to building site according to NPCR 013 Part B. The steel comes from two
different suppliers, and the scenario above represents the average transport of the steel
arriving at the customer in Norway.
EPD for the best environmental decision 4
End of Life (C1, C3, C4)
Unit Value
kg 0
Hazardous waste disposed
kg 0
Collected as mixed construction waste
kg 0
Reuse
kg 0,95
Recycling
kg 0
Energy recovery
kg 0,05
To landfill
Net new scrap is calculated by substracting the scrap content of outgoing steel from the
recycling rate. The scrap content is 37,4 % from suppliers. Note that outgoing scrap and the
parameter for Secondary Material content (SM) differ, wherein the latter accounts for the total
amount of scrap needed in the system to fulfill the declared unit.
A 95% recovery rate is assumed, wherein 5% is assumed landfilled - in effect providing a 95%
recycling rate. Reuse is not included in this scenario.
Transport to waste processing (C2)
Capacity utilisation Distance Fuel/Energy value
Type Type of vehicle
(incl. return) % KM consumption (l/t)
Waste collection 50 % Lorry 21t 19 0,4 7,4
Truck 26 % Lorry 16-32t EURO5 278 0,04 12,2
To provide a plausible scenario for transportation to waste processing, a study of Norwegian
waste treatment was used as proxy data (Raadal et al., 2009).
Benefits and loads beyond the system boundaries (D)
Unit Value
Steel waste kg -0,0576
Module D is calculated as net scrap * LCI for scrap, where the scrap LCI is calculated as the
credit for avoided primary production of steel, minus the burden of recycling steel scrap to
make new steel, multiplied by the process yield. LCI for scrap has been provided by worldsteel
(Eurofer, 2019; Worldsteel, 2017).
Additional technical information
Not relevant.
EPD for the best environmental decision 5
The LCA results are presented below for the declared unit defined on page 2 of the EPD
document. Impact assessment results are presented with core and additional impact indicators
presented in EN15804+A2. Reading example: 9,0 E-03 = 9,0*10-3 = 0,009
System boundaries (X=included, MND= module not declared, MNR=module not
relevant)
Benefits
& loads
Assembly
Product stage Use stage End of life stage beyond
stage
system
boundary
EPD for the best environmental decision 6
slairetam
waR
tropsnarT
gnirutcafunaM
tropsnarT ylbmessA
esU
ecnanetniaM
riapeR
tnemecalpeR tnemhsibrufeR
esu
ygrene
lanoitarepO
esu
retaw
lanoitarepO
noitilomed
noitcurtsnoc-eD
tropsnarT
gnissecorp
etsaW
lasopsiD
-gnilcyceR-yrevoceR-esueR
laitnetop
LCA: Results
A1 A2 A3 A4 A5 B1 B2 B3 B4 B5 B6 B7 C1 C2 C3 C4 D
X X X X MND MND MND MND MND MND MND MND X X X X X
Core environmental impact indicators
Indicator Unit A1-A3 A4 C1 C2 C3 C4 D
GWP-total kg CO2 eq. 2,00E+00 8,48E-02 2,14E-02 6,99E-02 2,12E-04 2,64E-04 -9,77E-01
GWP-fossil kg CO2 eq. 1,98E+00 8,47E-02 2,14E-02 6,97E-02 2,00E-04 2,63E-04 -9,76E-01
GWP-biogenic kg CO2 eq. 1,58E-02 7,85E-05 1,85E-05 1,46E-04 1,21E-05 9,28E-07 -6,32E-04
GWP-LULUC kg CO2 eq. 8,80E-04 1,30E-05 2,14E-06 2,02E-05 5,41E-07 2,49E-07 1,41E-04
kg CFC11
ODP 1,40E-07 9,57E-09 4,58E-09 1,58E-08 2,13E-11 1,07E-10 -5,31E-16
eq.
AP mol H⁺ eq. 8,57E-03 1,28E-03 2,23E-04 3,30E-04 1,63E-06 2,48E-06 -1,75E-03
EP-
kg P eq. 9,16E-05 2,59E-07 7,10E-08 3,64E-07 6,73E-09 2,76E-09 -2,00E-07
freshwater
EP-marine kg N eq. 1,62E-03 3,71E-04 9,85E-05 1,17E-04 4,45E-07 8,56E-07 -2,61E-04
EP-terrestial mol N eq. 1,87E-02 4,07E-03 1,08E-03 1,29E-03 5,02E-06 9,42E-06 -2,55E-03
kg NMVOC
POCP 7,75E-03 1,05E-03 2,97E-04 4,24E-04 1,44E-06 2,74E-06 -1,34E-03
eq.
ADP-M&M kg Sb eq. 2,31E-05 8,89E-08 1,10E-08 1,81E-07 1,22E-08 6,01E-10 -2,07E-06
-
ADP-fossil MJ 2,20E+01 1,16E+00 2,94E-01 1,01E+00 2,90E-03 7,35E-03
8,50E+00
WDP m³ 3,63E-01 1,91E-03 4,19E-04 2,17E-03 1,05E-04 3,30E-04 -1,11E-01
GWP-total: Global Warming Potential; GWP-fossil: Global Warming Potential fossil fuels; GWP-biogenic:
Global Warming Potential biogenic; GWP-LULUC: Global Warming Potential land use and land use change;
ODP: Depletion potential of the stratospheric ozone layer;
AP: Acidification potential, Accumulated Exceedance; EP-freshwater: Eutrophication potential, fraction of
nutrients reaching freshwater end compartment; See “additional Norwegian requirements” for indicator
given as PO4 eq. EP-marine: Eutrophication potential, fraction of nutrients reaching freshwater end
compartment; EP-terrestial: Eutrophication potential, Accumulated Exceedance; POCP: Formation
potential of tropospheric ozone; ADP-M&M: Abiotic depletion potential for non-fossil resources (minerals
and metals); ADP-fossil: Abiotic depletion potential for fossil resources; WDP: Water deprivation potential,
deprivation weighted water counsumption
Additional environmental impact indicators
Indicator Unit A1-A3 A4 C1 C2 C3 C4 D
Disease 1,27E-07 1,10E-08 5,90E-09 6,39E-09 2,73E-11 4,85E-11 -2,96E-08
PM
incidence
4,88E-02 2,75E-03 1,25E-03 4,38E-03 3,80E-05 3,01E-05 2,56E-02
IRP kBq U235 eq.
4,86E+01 4,90E-01 1,72E-01 7,14E-01 6,68E-03 4,64E-03 3,72E-02
ETP-fw CTUe
1,63E-08 3,30E-11 6,65E-12 2,06E-11 8,30E-13 1,18E-13 2,92E-10
HTP-c CTUh
4,13E-08 7,51E-10 1,25E-10 6,91E-10 8,45E-12 3,05E-12 -1,31E-08
HTP-nc CTUh
9,17E+00 5,86E-01 3,74E-02 5,36E-01 1,73E-02 1,54E-02 2,15E-01
SQP Dimensionless
PM: Particulate matter emissions; IRP: Ionising radiation, human health; ETP-fw: Ecotoxicity (freshwater);
ETP-c: Human toxicity, cancer effects; HTP-nc: Human toxicity, non-cancer effects; SQP: Land use related
impacts / soil quality
Classification of disclaimers to the declaration of core and additional environmental
impact indicators
ILCD
Indicator Disclaimer
classification
Global warming potential (GWP) None
ILCD type / level
Depletion potential of the stratospheric ozone layer (ODP) None
1
Potential incidence of disease due to PM emissions (PM) None
Acidification potential, Accumulated Exceedance (AP) None
Eutrophication potential, Fraction of nutrients reaching marine end
None
compartment (EP-marine)
ILCD type / level
Eutrophication potential, Accumulated Exceedance (EP-terrestrial) None
2
Formation potential of tropospheric ozone (POCP) None
Potential Human exposure efficiency relative to U235 (IRP) 1
Abiotic depletion potential for non-fossil resources (ADP-minerals&metals) 2
Abiotic depletion potential for fossil resources (ADP-fossil) 2
Water (user) deprivation potential, deprivation-weighted water consumption
2
(WDP)
ILCD type / level
Potential Comparative Toxic Unit for ecosystems (ETP-fw) 2
3
Potential Comparative Toxic Unit for humans (HTP-c) 2
Potential Comparative Toxic Unit for humans (HTP-nc) 2
Potential Soil quality index (SQP) 2
EPD for the best environmental decision 7
Disclaimer 1 – This impact category deals mainly with the eventual impact of low dose ionizing radiation on
human health of the nuclear fuel cycle. It does not consider effects due to
possible nuclear accidents, occupational exposure nor due to radioactive waste disposal in underground facilities.
Potential ionizing radiation from the soil, from radon and from some
construction materials is also not measured by this indicator.
Disclaimer 2 – The results of this environmental impact indicator shall be used with care as the uncertainties on
these results are high or as there is limited experienced with the indicator
Resource use
Parameter Unit A1-A3 A4 C1 C2 C3 C4 D
1,72E+00 7,70E-03 1,65E-03 1,15E-02 1,52E-02 6,27E-05 7,00E-02
RPEE MJ
7,22E-03 0,00E+00 0,00E+00 0,00E+00 0,00E+00 0,00E+00 0,00E+00
RPEM MJ
1,73E+00 7,70E-03 1,65E-03 1,15E-02 1,52E-02 6,27E-05 7,00E-02
TPE MJ
2,21E+01 1,16E+00 2,94E-01 1,01E+00 2,90E-03 7,36E-03 -8,50E+00
NRPE MJ
0,00E+00 0,00E+00 0,00E+00 0,00E+00 0,00E+00 0,00E+00 0,00E+00
NRPM MJ
2,21E+01 1,16E+00 2,94E-01 1,01E+00 2,90E-03 7,36E-03 -8,50E+00
TRPE MJ
3,83E-01 0,00E+00 0,00E+00 0,00E+00 0,00E+00 0,00E+00 0,00E+00
SM kg
0,00E+00 0,00E+00 0,00E+00 0,00E+00 0,00E+00 0,00E+00 0,00E+00
RSF MJ
0,00E+00 0,00E+00 0,00E+00 0,00E+00 0,00E+00 0,00E+00 0,00E+00
NRSF MJ
1,52E-02 6,25E-05 1,48E-05 1,09E-04 1,11E-04 7,83E-06 -4,30E-03
W m3
RPEE Renewable primary energy resources used as energy carrier; RPEM Renewable primary energy
resources used as raw materials; TPE Total use of renewable primary energy resources; NRPE Non
renewable primary energy resources used as energy carrier; NRPM Non renewable primary energy
resources used as materials; TRPE Total use of non renewable primary energy resources; SM Use of
secondary materials; RSF Use of renewable secondary fuels; NRSF Use of non renewable secondary fuels; W
Use of net fresh water
End of life - Waste
Parameter Unit A1-A3 A4 C1 C2 C3 C4 D
6,44E-03 3,13E-05 8,57E-06 4,48E-05 9,39E-07 5,73E-07 0,00E+00
HW kg
1,03E+00 4,68E-02 3,92E-04 3,75E-02 1,04E-04 5,00E-02 0,00E+00
NHW kg
6,43E-05 4,18E-06 2,03E-06 6,90E-06 2,35E-08 4,82E-08 0,00E+00
RW kg
HW Hazardous waste disposed; NHW Non hazardous waste disposed; RW Radioactive waste disposed
End of life – output flow
Parameter Unit A1-A3 A4 C1 C2 C3 C4 D
0,00E+00 0,00E+00 0,00E+00 0,00E+00 0,00E+00 0,00E+00 0,00E+00
CR kg
1,80E-02 0,00E+00 0,00E+00 0,00E+00 9,50E-01 0,00E+00 0,00E+00
MR kg
0,00E+00 0,00E+00 0,00E+00 0,00E+00 0,00E+00 0,00E+00 0,00E+00
MER kg
0,00E+00 0,00E+00 0,00E+00 0,00E+00 0,00E+00 0,00E+00 0,00E+00
EEE MJ
0,00E+00 0,00E+00 0,00E+00 0,00E+00 0,00E+00 0,00E+00 0,00E+00
ETE MJ
CR Components for reuse; MR Materials for recycling; MER Materials for energy recovery; EEE Exported
electric energy; ETE Exported thermal energy
EPD for the best environmental decision 8
Information describing the biogenic carbon content at the factory gate
Biogenic carbon content Unit Value
Biogenic carbon content in product kg C 0,00E+00
Biogenic carbon content in the accompanying packaging kg C 0,00E+00
Additional Norwegian requirements
Greenhous gas emission from the use of electricity in the manufacturing phase
National production mix from import, low voltage (production of transmission lines, in addition
to direct emissions and losses in grid) of applied electricity for the manufacturing prosess(A3).
National electricity grid Unit Value
Ecoinvent v3.8- Lithuania kg CO2 -eq/kWh 0,548
Additional environmental impact indicators required in NPCR Part A for construction
products
In order to increase the transparency of biogenic carbon contribution to climate impact, the
indicator GWP-IOBC is required as it declares climate impacts calculated according to the
principle of instantanious oxidation. GWP-IOBC is also reffered to as GWP-GHG in context to
Swedish public procurement legislation.
Indicator Unit A1-A3 A4 C1 C2 C3 C4 D
GWP-IOBC kg CO2 eq. 2,00E+00 8,48E-02 2,14E-02 6,99E-02 2,12E-04 2,64E-04 -9,77E-01
GWP-IOBC Global warming potential calculated according to the principle of instantanious oxidation.
Hazardous substances
The declaration is based upon reference to threshold values and/or test results and/or material
safety data sheets provided to EPD verifiers. Documentation available upon request to EPD
owner.
■ The product contains no substances given by the REACH Candidate list or the
Norwegian priority list.
□ The product contains substances given by the REACH Candidate list or the Norwegian
priority list that are less than 0,1 % by weight.
□ The product contain dangerous substances, more then 0,1% by weight, given by the
REACH Candidate List or the Norwegian Priority list, see table.
□ The product contains no substances given by the REACH Candidate list or the
Norwegian priority list. The product is classified as hazardous waste (Avfallsforskiften,
Annex III), see table.
Indoor environment
No tests have been carried out on the product concerning indoor climate - Not relevant.
Carbon footprint
Carbon footprint has not been worked out for the product.
EPD for the best environmental decision 9
Bibliography
ISO 14025:2010 Environmental labels and declarations - Type III environmental
declarations - Principles and procedures
ISO 14044:2006 Environmental management - Life cycle assessment -
Requirements and guidelines
EN 15804:2012+A2:2019 Sustainability of construction works - Environmental product
declaration - Core rules for the product category of construction
products. Issued 12.01.2019
ISO 21930:2007 Sustainability in building construction - Environmental
declaration of building products
Johansen (2023) Life cycle assessment (LCA) report for steel core piles.
Ferrometall AS
NPCR PART A Construction Products and Services. Version 2.0, issued
24.03.2021, EPD Norway
NPCR 013 Part B for Steel and Aluminium products. Version 4.0, issued
06.10.2021, EPD Norway
Raadal et al. (2009) Klimaregnskap for avfallshåndtering. Fase I og II:
Glassemballasje, metallemballasje, papir, papp, plastemballasje,
våtorganisk avfall, treavfall og restavfall fra husholdninger. ISBN:
82-8035-073-X.
Program Operator tlf +47 23 08 80 00
The Norwegian EPD Foundation
Post Box 5250 Majorstuen, 0303 Oslo e-post: post@epd-norge.no
Norway web www.epd-norge.no
Publisher tlf +47 23 08 80 00
The Norwegian EPD Foundation
Post Box 5250 Majorstuen, 0303 Oslo e-post: post@epd-norge.no
Norway web www.epd-norge.no
Owner of the decleration tlf +47 32 89 10 30
Ferometall AS Fax
Gyldenløves plass 1, 3044 Drammen e-post: info@ferrometall.no
Norway web ferrometall.no
Author of the life cycle assesment tlf +47 41 79 94 17
Dan André Johansen Fax
Asplan Viak AS e-post: asplanviak@aplanviak.no
Abels gate 9, 7030 Trondheim,
web www.asplanviak.no
Norway
ECO Platform web www.eco-platform.org
ECO Portal web ECO Portal
EPD for the best environmental decision 10
EPD for the best
environmental
decision
The Norwegian EPD foundation
www.epd-norge.no
EPD for the best environmental decision 11
