ENVIRONMENTAL PRODUCT DECLARATION
as per ISO 14025 and EN 15804+A2
Owner of the Declaration Stiferite
Publisher Institut Bauen und Umwelt e.V. (IBU)
Programme holder Institut Bauen und Umwelt e.V. (IBU)
Declaration number EPD-STF-20220333-CBC2-EN
Issue date 16.02.2023
Valid to 15.02.2028
Stiferite ISOVENTILATO average thick panel
Stiferite
www.ibu-epd.com | https://epd-online.com
General Information
Stiferite Stiferite ISOVENTILATO average thick panel
Programme holder Owner of the declaration
IBU – Institut Bauen und Umwelt e.V. Stiferite
Hegelplatz 1 Viale Navigazione Interna 54
10117 Berlin 35129 Padova
Germany Italy
Declaration number Declared product / declared unit
EPD-STF-20220333-CBC2-EN Stiferite ISOVENTILATO average thick panel expanded rigid polyurethane
foam, covered on one side by mineral fiber glass and on one side by a
facer which gives waterproof property (0,2 bar) and permeable to vapour
and Isoventilato board has two wooden (OSB3) laths along the entire
length upper face, and produced by Stiferite. The EPD applies to 1 m2 of
110 mm thick PUR sandwich board, i.e. 0.11 m3, with an average density
between foam and facing of 43.5 kg/m3.
This declaration is based on the product category rules: Scope:
Insulating materials made of foam plastics, 01.08.2021 Stiferite produces Stiferite ISOVENTILATO which is a high performance
(PCR checked and approved by the SVR) insulation board manufactured from closed cell expanded rigid
polyurethane foam, covered on one side by mineral fiber glass and on one
side by a facer which gives waterproof property (0,2 bar) and permeable to
Issue date vapour and Isoventilato board has two wooden (OSB3) laths along the
entire length upper face. The data have been provided by the only Stiferite
16.02.2023
factory that is located in Padova (Italy) for the year 2021 and sold
worldwide.
The owner of the declaration shall be liable for the underlying information
Valid to
and evidence; the IBU shall not be liable with respect to manufacturer
15.02.2028 information, life cycle assessment data and evidences.
The EPD was created according to the specifications of EN 15804+A2. In
the following, the standard will be simplified as EN 15804.
Verification
The standard EN 15804 serves as the core PCR
Independent verification of the declaration and data according to ISO
14025:2011
internally X externally
Dipl.-Ing. Hans Peters
(Chairman of Institut Bauen und Umwelt e.V.)
Dipl.-Ing. Hans Peters Prof. Dr. Birgit Grahl,
(Managing Director Institut Bauen und Umwelt e.V.) (Independent verifier)
1 Environmental Product Declaration - Stiferite - Stiferite ISOVENTILATO average thick panel
Product
Association (EU/EFTA) (with the exception of Switzerland)
Product description/Product definition Regulation (EU) No.305/2011 (CPR) applies. The product
Stiferite's thermal insulation panels are mainly used in the needs a Declaration of Performance taking into consideration
building/construction sector and in industrial insulation. EN 13165:2012+A2:2016. Thermal insulation products for
The panels are made of thermo-setting closed cells building- factory made rigid polyurethane foam (PU) products -
polyurethane foam (PU) supplied with various types of flexible Specification and the CE-marking. For the application and use
facers on both sides of the panel. The nature/type of facer is a the respective national provisions apply.
function of the type of panel and its application.
Expanded rigid polyurethane foam is distinguished by its Base materials/Ancillary materials
thermal insulation performance, mechanical resistance, Core material (about 96.8 % of the weight of the declared
workability, lightness, and durability. unit): Closed-cell Polyiso (PIR) rigid foam made from MDI (50-
The performance of Stiferite's panels is determined based on 65 %), polyols (20-30 %), pentane (4-6 %) and additives (4-6
the European norm EN13165:2012+A2:2016 Thermal %).
insulation products for buildings - Factory-made rigid Facing (about 3.21 % of the weight of the declared unit):
polyurethane foam (PU) products - Specification. consisting of glass fiber (20-30 %), calcium carbonate (35-45
This EPD refers to Stiferite's ISOVENTILATO average thick %), polypropylene (20-30 %) and graphite (10-20 %).
panel, made of an insulation component in polyurethane foam
using blowing agent Pentanebased, covered on one side by The PU board for insulation:
mineral fiber glass and on one side by a facer which gives
• This product/article/at least one partial article contains
waterproof property (0,2 bar) and permeable to vapour and
substances listed in the candidate list (date: 17.01.2022)
Isoventilato board has two wooden (OSB3) laths along the
exceeding 0.1 percentage by mass: no
entire length upper face.
The panel is produced in standard dimensions of 1200 x 2400 • This product/article/at least one partial article doesn't
mm and straight finish borders. contain other carcinogenic, mutagenic, reprotoxic
Upon request and for minimum quantities, the panels may be (CMR) substances in categories 1A or 1B which are not
produced in various dimensions, and the borders may be on the candidate list, exceeding 0.1 percentage by
rabbeted along the sides. The surface of the panel may be mass: no
evened out with sandpaper in order to allow installation on • Biocide products were added to this construction
uneven surfaces. Stiferite ISOVENTILATO panel is produced product or it has been treated with biocide products (this
by a certified company with systems:ISO 9001, ISO 45001, ISO then concerns a treated product as defined by the (EU)
14001 in its entire line of products. Ordinance on Biocide Products No.528/2012): no
Application
Additional declaration according to quoted law: The product is
The Stiferite ISOVENTILATO panel is suitable for insulating: compliant with all requirements indicated in chapter 2.5.7
Pitched roofs: with Isoventilato system, ventilated, under roof 'Isolanti termici ed acustici' of the n.256 D.L. of the 23th June
tiles, pantiles and sheet-metal Walls: application from the inside 2022 (CAM EDILIZIA):
or outside, behind the facings
• Any blowing agent with Ozone depletion potential >0 is
Technical Data not used in production
In this Life Cycle Assessment, a PU insulation board with the • Any substances of Very High Concern-SVHC in
following properties has been regarded: concentration of more than 0,1 %w are not used in
production (REACH n. 1907/2006). Any specific
Constructional data
authorizations for use are eserved provided for by the
Name Value Unit same Regulation for the substances included in Annex
Gross density 43.5 kg/m3 XIV and specifications restrictions set out in Annex XVII
of the Regulation.
Declared Average Thermal conductivity λD acc.
0.026 W/mK • Catalysts lead-based are not used in production
to EN 13165
• Flame retardants used in production (belonging to the
Compressive strength at 10% deformation acc. to
>150 kPa Organophosphorus class) are not banned by any
EN 826
national or European regulation
Tensile strength perpendicular to the face acc. to >35 kPa • According to the raw materials declarations of suppliers,
EN 1607 the minimum amount of recycled raw materials based
Water absorption by total immersion acc. to EN Vol.- on the insulation board (PU foam and facers) weight is 3
<2
12087 % % and the minimum amount of recycled raw materials
w
Water absorption by partial immersion acc. to EN based on the PU insulation foam weight is 4 % in
< 0.1 kg/m² w
1609 compliance with REMADE in Italy type 1 certification
Water vapour diffusion resistance factor μ acc. to (note: this information is not explicitly considered in the
56
EN 12086 LCA and not included in the EPD tables that only refer
Euroclass reaction to fire acc. to EN 11925 E to recycling content in the foreground system).
This provides a thermal resistance R = 4.2 m² k/W. Reference service life
The durability of insulation panels is normally at least as long as
Product according to the CPR based on a
the lifetime of the building in which it is used. The experimental
hEN/:13165:2012+A2:2016 For the placing on the market of the
data show that the reference life is greater than 50 years.
product in the European Union/European Free Trade
LCA: Calculation rules
2 Environmental Product Declaration - Stiferite - Stiferite ISOVENTILATO average thick panel
thermal insulation board. The life cycle is split into the following
Declared Unit individual phases:
The declared unit is 1 m² with a thickness of 110 mm, e. g. 0.11 A1 - Raw material formulation
m³. A2 - Raw material transport
Corresponding conversion factors are listed in the table below. A3 - Production of the insulation board and packaging material
Declared unit A4 - Transport to the construction site
C1 - demolition and deconstruction
Name Value Unit
C2 - Transport to end of life
Declared unit 1 m2 C3 - End-of-Life: waste management (thermal recovery)
Gross density 43.5 kg/m3 C4 - End-of-Life: waste management (landfill)
Grammage 4.77 kg/m2 D - Benefits and loads beyond system boundary
Layer thickness 0.11 m Geographic Representativeness
Declared average thermal conductivity λD 0.026 W/mK Land or region, in which the declared product system is
manufactured, used or handled at the end of the product´s
This provides a thermal resistance R = 4.2 m² /W.
lifespan: Italy
Comparability
System boundary
Basically, a comparison or an evaluation of EPD data is only
Type of the EPD: cradle to gate - with options
possible if all the data sets to be compared were created
This life cycle assessment for the production of the
according to EN 15804 and the building context, respectively
polyurethane insulation board considers the life cycle from the
the product-specific characteristics of performance, are taken
supply of raw materials to the manufacturer´s gate (cradle-to-
into account. The background database used is GaBi 2022
gate with options). It also includes the transport to the
database (v. 2022.1)
construction site and the end-of-life stage of the used PU
LCA: Scenarios and additional technical information
Name Value Unit
Characteristic product properties of biogenic carbon
Cardboard 0.00691 kg
EPS stock 0.00578 kg
Information on describing the biogenic Carbon Content at
EPS stock - glue 0.00041 kg
factory gate
Paper labels 0.00014 kg
Name ValueUnit
PE film 0.06123 kg
kg
Biogenic carbon content in product 0.42 PP tape 0.00005 kg
C
PUR stucks 0 kg
Biogenic carbon content in accompanying kg
packaging 0.003 C SBR labels 0.00001 kg
TOTAL PACKAGING 0.07454 kg
The following technical scenario information is required for the
declared modules and optional for non-declared modules.
End of life (C1-C4)
Modules for which no information is declared can be deleted;
Name Value Unit
additional information can also be listed if necessary.
Scenario No 1: Material Incineration 100 %
The following technical information is a basis for the declared Scenario No 2: Landfill 100 %
modules or can be used for developing specific scenarios in the
C1 – Deconstruction and demolition (0.2 MJ/kg as electrical
context of a building assessment if modules are not declared
consumption assumed)
(MND).
C2 – Panelis transported from the building site to a treatment
A5 is not declared including the disposal of the packaging
plant by truck and an average distance of 100 km is
material on the construction site, the amounts of packaging
considered.
materials included in the LCA calculations must be declared as
technical scenario information for Module A5.
C3/C4- Disposal scenarios used are divided into 2 sub-
scenarios:
1) Incineration 100 % (C3/1)
Transport to the building site (A4) 2) Landfilling 100 % (C4/2)
Name Value Unit
Truck with a capacity of 17.3 tons 298 km Reuse, recovery and/or recycling potentials (D), relevant
Ferry with a capacity of 1200-10000 dwt payload scenario information
0.0219 km
capacity D: Benefits and loads beyond system boundary are divided into
Ship with a capacity of 27500 dwt payload 2 sub-scenarios:
0 km
capacity tons Name Value Unit
Plane with a capacity of 22 ton 0 km Scenario No 1: Material Incineration 100 %
Scenario No 2: Landfill 100 %
Type and amount of packaging included in module A3
3 Environmental Product Declaration - Stiferite - Stiferite ISOVENTILATO average thick panel
LCA: Results
The tables below show the results of the LCA. Basic information on all declared modules provides chapter 4.
There are two scenarios for the end-of-life (C2, C4 and D) analyzed: Scenario 1 considers 100 % incineration, Scenario 2 considers
100 % landfill disposal.
For SM, RSF, NRSF, CRU indicators only the foreground system is considered.
DESCRIPTION OF THE SYSTEM BOUNDARY (X = INCLUDED IN LCA; ND = MODULE OR INDICATOR NOT DECLARED; MNR =
MODULE NOT RELEVANT)
Benefits and
Construction loads beyond
Product stage Use stage End-of-life stage
process stage the system
boundaries
la ire ta m w a Ry lp p u s tro p s n a rT g n iru tc a fu n a M e h t m o rf tro p s n a rTe tis e h t o t e ta g y lb m e s s A e s U e c n a n e tn ia M ria p e R tn e m e c a lp e R tn e m h s ib ru fe R y g re n e la n o ita re p Oe s u re ta w la n o ita re p Oe s u n o itc u rts n o c -e Dn o itilo m e d tro p s n a rT g n is s e c o rp e ts a W la s o p s iD -e s u e R-y re v o c e R-g n ilc y c e Rla itn e to p
A1 A2 A3 A4 A5 B1 B2 B3 B4 B5 B6 B7 C1 C2 C3 C4 D
X X X X MND MND MND MNR MNR MNR MND MND X X X X X
RESULTS OF THE LCA - ENVIRONMENTAL IMPACT according to EN 15804+A2: 1 m2 ISOVENTILATO
Parameter Unit A1-A3 A4 C1 C2 C3/1 C3/2 C4/1 C4/2 D/1 D/2
GWP-total kg CO 2 eq 9.15E+00 1.22E-01 1.09E-01 2.89E-02 9.85E+00 0 0 -7.31E-02 -4.15E+00 0
GWP-fossil kg CO 2 eq 1.11E+01 1.21E-01 1.09E-01 2.86E-02 8.09E+00 0 0 -7.31E-02 -4.15E+00 0
GWP-
biogenic kg CO 2 eq -1.92E+00 3.94E-04 6.43E-05 9.27E-05 1.76E+00 0 0 -4.32E-05 -3.69E-03 0
GWP-luluc kg CO 2 eq 5.47E-03 8.18E-04 7.06E-06 1.92E-04 2.31E-05 0 0 -4.74E-06 -2.26E-04 0
ODP kg CFC11 eq 1.53E-11 1.19E-14 1.08E-12 2.8E-15 7.16E-13 0 0 -7.22E-13 -3.08E-11 0
AP mol H+ eq 2.15E-02 4.31E-04 1.6E-04 9.54E-05 5.7E-03 0 0 -1.07E-04 -5.16E-03 0
EP-
kg P eq 3.92E-05 4.34E-07 4.89E-08 1.02E-07 2.16E-07 0 0 -3.28E-08 -1.46E-06 0
freshwater
EP-marine kg N eq 5.94E-03 1.99E-04 4.37E-05 4.36E-05 2.72E-03 0 0 -2.93E-05 -1.5E-03 0
EP-terrestrial mol N eq 6.2E-02 2.22E-03 4.67E-04 4.88E-04 3.16E-02 0 0 -3.14E-04 -1.61E-02 0
kg NMVOC
POCP 2.25E-02 3.88E-04 1.23E-04 8.56E-05 6.98E-03 0 0 -8.29E-05 -4.27E-03 0
eq
ADPE kg Sb eq 3.1E-06 1.22E-08 1.3E-08 2.88E-09 2.81E-08 0 0 -8.69E-09 -4.19E-07 0
ADPF MJ 2.79E+02 1.59E+00 2.31E+00 3.75E-01 2.87E+00 0 0 -1.55E+00 -8.26E+01 0
m3 world eq
WDP 2.05E+00 1.36E-03 8.13E-03 3.19E-04 9.36E-01 0 0 -5.46E-03 -2.35E-01 0
deprived
GWP = Global warming potential; ODP = Depletion potential of the stratospheric ozone layer; AP = Acidification potential of land and water; EP =
Eutrophication potential; POCP = Formation potential of tropospheric ozone photochemical oxidants; ADPE = Abiotic depletion potential for non-fossil
resources; ADPF = Abiotic depletion potential for fossil resources; WDP = Water (user) deprivation potential)
RESULTS OF THE LCA - INDICATORS TO DESCRIBE RESOURCE USE according to EN 15804+A2: 1 m2 ISOVENTILATO
Parameter Unit A1-A3 A4 C1 C2 C3/1 C3/2 C4/1 C4/2 D/1 D/2
PERE MJ 2.2E+01 1.1E-01 3.34E-01 2.6E-02 1.76E+01 0 0 -2.24E-01 -9.61E+00 0
PERM MJ 1.72E+01 ND ND ND -1.71E+01 0 0 ND ND 0
PERT MJ 3.93E+01 1.1E-01 3.34E-01 2.6E-02 4.36E-01 0 0 -2.24E-01 -9.61E+00 0
PENRE MJ 1.78E+02 1.6E+00 2.31E+00 3.76E-01 1.01E+02 0 0 -1.55E+00 -8.26E+01 0
PENRM MJ 1.02E+02 ND ND ND -9.85E+01 0 0 ND ND 0
PENRT MJ 2.79E+02 1.6E+00 2.31E+00 3.76E-01 2.87E+00 0 0 -1.55E+00 -8.26E+01 0
SM kg 3.38E-01 ND ND ND ND 0 0 ND ND 0
RSF MJ ND ND ND ND ND 0 0 ND ND 0
NRSF MJ ND ND ND ND ND 0 0 ND ND 0
FW m3 6.96E-02 1.28E-04 5.06E-04 3E-05 2.2E-02 0 0 -3.39E-04 -1.46E-02 0
PERE = Use of renewable primary energy excluding renewable primary energy resources used as raw materials; PERM = Use of renewable primary
energy resources used as raw materials; PERT = Total use of renewable primary energy resources; PENRE = Use of non-renewable primary energy
excluding non-renewable primary energy resources used as raw materials; PENRM = Use of non-renewable primary energy resources used as raw
materials; PENRT = Total use of non-renewable primary energy resources; SM = Use of secondary material; RSF = Use of renewable secondary fuels;
NRSF = Use of non-renewable secondary fuels; FW = Use of net fresh water
RESULTS OF THE LCA – WASTE CATEGORIES AND OUTPUT FLOWS according to EN 15804+A2:
1 m2 ISOVENTILATO
Parameter Unit A1-A3 A4 C1 C2 C3/1 C3/2 C4/1 C4/2 D/1 D/2
HWD kg 7.58E-08 8.46E-12 1.65E-10 1.99E-12 3.42E-10 0 0 -1.11E-10 -7.74E-09 0
NHWD kg 2.45E-01 2.61E-04 4.91E-04 6.13E-05 1.11E-01 0 0 -3.29E-04 -1.83E-02 0
RWD kg 3.34E-03 2.97E-06 3.84E-04 6.98E-07 1.22E-04 0 0 -2.58E-04 -1.1E-02 0
CRU kg ND ND ND ND ND 0 0 ND ND 0
4 Environmental Product Declaration - Stiferite - Stiferite ISOVENTILATO average thick panel
MFR kg ND ND ND ND ND 0 0 ND ND 0
MER kg ND ND ND ND ND 0 0 ND ND 0
EEE MJ ND ND ND ND 2.47E+01 0 0 ND ND 0
EET MJ ND ND ND ND 1.42E+01 0 0 ND ND 0
HWD = Hazardous waste disposed; NHWD = Non-hazardous waste disposed; RWD = Radioactive waste disposed; CRU = Components for re-use;
MFR = Materials for recycling; MER = Materials for energy recovery; EEE = Exported electrical energy; EET = Exported thermal energy
RESULTS OF THE LCA – additional impact categories according to EN 15804+A2-optional:
1 m2 ISOVENTILATO
Parameter Unit A1-A3 A4 C1 C2 C3/1 C3/2 C4/1 C4/2 D/1 D/2
Disease
PM 1.77E-07 2.5E-09 1.43E-09 5.46E-10 1.7E-08 0 0 -9.59E-10 -4.57E-08 0
incidence
IR kBq U235 eq 3.93E-01 4.48E-04 5.62E-02 1.05E-04 1.79E-02 0 0 -3.77E-02 -1.61E+00 0
ETP-fw CTUe 1.15E+02 1.13E+00 7.07E-01 2.65E-01 9.45E-01 0 0 -4.75E-01 -2.04E+01 0
HTP-c CTUh 1.26E-08 2.33E-11 1.3E-11 5.47E-12 6.64E-11 0 0 -8.74E-12 -4.99E-10 0
HTP-nc CTUh 5.51E-07 1.45E-09 6.62E-10 3.35E-10 2.47E-09 0 0 -4.45E-10 -2.42E-08 0
SQP SQP 1.03E+02 6.74E-01 2.12E-01 1.59E-01 5.35E-01 0 0 -1.42E-01 -6.1E+00 0
PM = Potential incidence of disease due to PM emissions; IR = Potential Human exposure efficiency relative to U235; ETP-fw = Potential comparative
Toxic Unit for ecosystems; HTP-c = Potential comparative Toxic Unit for humans (cancerogenic); HTP-nc = Potential comparative Toxic Unit for humans
(not cancerogenic); SQP = Potential soil quality index
Disclaimer 1 – for the indicator “Potential Human exposure efficiency relative to U235”. This impact category deals mainly with the
eventual impact of low-dose ionizing radiation on human health of the nuclear fuel cycle. It does not consider effects due to possible
nuclear accidents, occupational exposure or radioactive waste disposal in underground facilities. Potential ionizing radiation from the
soil, radon and from some construction materials is also not measured by this indicator.
Disclaimer 2 – for the indicators “abiotic depletion potential for non-fossil resources”, “abiotic depletion potential for fossil resources”,
“water (user) deprivation potential, deprivation-weighted water consumption”, “potential comparative toxic unit for ecosystems”,
“potential comparative toxic unit for humans – cancerogenic”, “Potential comparative toxic unit for humans - not cancerogenic”,
“potential soil quality index”. The results of this environmental impact indicator shall be used with care as the uncertainties on these
results are high as there is limited experience with the indicator.
References
Standards EN 13165:2012+A2:2016 Thermal insulation products for
buildings - Factory made rigid polyurethane foam (PU)
CPR products -Specification
Regulation (EU) No.305/2011 laying down harmonised
conditions for the marketing of construction products and EN 15804
repealing Council Directive 89/106/EEC EN 15804:2012+A2:2019+AC:2021 Sustainability of
construction works — Environmental Product Declarations —
EN 826 Core rules forthe product category of construction products.
EN 826:2013 Determination of Compression Behavior of
Thermal Insulation Products ISO 9001
ISO 9001:2015 Quality management
EN 1607
EN 1607: 2013 Thermal insulating products for building ISO 14001
applications. Determination of tensile strength perpendicular to ISO 14001: 2015 Environmental management systems
faces
ISO 14025
EN 1609 EN ISO 14025:2011 Environmental labels and declarations —
EN 1609: Thermal insulating products for building applications. Type III environmental declarations - Principles and procedures.
Determination of short term water absorption by partial
immersion. ISO 45001
ISO 45001: 2018 Occupational health and safety management
EN 11925 systems
EN 11925:2010 Reaction to fire tests. Ignitability of products
subjected to direct impingement of flame. Single-flame source GaBi 2022
test. GaBi 10 and DB 2022.1: Documentation of GaBi 10: Software-
System and Database for Life Cycle Engineering. Copyright,
EN 12086 TM. Stuttgart, Leinfelden-Echterdingen, 1992-2022
EN 12086: 2013 Thermal insulating products for building http://www.gabi-software.com
applications. Determination of water vapour transmission
properties. IBU 2021
Institut Bauen und Umwelt e.V.: General Instructions for the
EN 12087 EPD programme of Institut Bauen und Umwelt e.V., Version
EN 12087:2013 Thermal insulating products for building 2.0, Berlin: Institut Bauen und Umwelt e.V., 2021
applications. Determination of long term water absorption by www.ibu-epd.com
immersion.
EN 13165 IBU PCR Part A
5 Environmental Product Declaration - Stiferite - Stiferite ISOVENTILATO average thick panel
Product Category Rules for Building-Related Products and criteri-minini-ambientali-cam
Services. Part A: Calculation Rules for the Life Cycle
Assessment and Requirements on the Project Report according REACH
to EN 15804+A2:2019; V1.2, 11/2021 REACH Registration, Evaluation, Authorization and Restriction
of Chemical, 2007
IBU PCR Part B
PCR Guidance-Texts for Building-Related Products and Ordinance on Biocide Products
Services; Part B: Requirements on the EPD for Insulating Regulation (eu) n. 528/2012 of the European Parliament and of
materials made of foam plastics; Institute Construction and the Council of 22 May 2012 concerning the making available on
Environment e.V. (IBU). Version 01.2019 the market and use of biocidal products Text with EEA
https://epd-online.com relevance
PANGPP 2022 REMADE IN ITALY
Piano d' Azione Nazionale sul Green Public Procurement Certificate No.1245/001 for Stiferite Rev. n. 0 18 November
(PANGPP) – Decreto Ministeriale n. 256 del 23-06-2022 2021
Gazzetta Ufficiale della Repubblica Italiana, Serie Generale
n.183 del 06-08-2022 https://www.mite.gov.it/notizie/novita-sui- STIFERITE LCA tool background report v 2.3 (03-06-2022)
6 Environmental Product Declaration - Stiferite - Stiferite ISOVENTILATO average thick panel
Publisher
Institut Bauen und Umwelt e.V. +49 (0)30 3087748- 0
Hegelplatz 1 info@ibu-epd.com
10117 Berlin www.ibu-epd.com
Germany
Programme holder
Institut Bauen und Umwelt e.V. +49 (0)30 3087748- 0
Hegelplatz 1 info@ibu-epd.com
10117 Berlin www.ibu-epd.com
Germany
Author of the Life Cycle Assessment
Sphera Solutions GmbH +49 711 341817-0
Hauptstraße 111- 113 info@sphera.com
70771 Leinfelden-Echterdingen www.sphera.com
Germany
Owner of the Declaration
Stiferite +39 049 8997911
Viale Navigazione Interna 54 info@stiferite.com
35129 Padova www.stiferite.com
Italy
7 Environmental Product Declaration - Stiferite - Stiferite ISOVENTILATO average thick panel
