ENVIRONMENTAL PRODUCT DECLARATION
as per ISO 14025 and EN 15804+A2
Owner of the Declaration Sto Scandinavia AB
Publisher Institut Bauen und Umwelt e.V. (IBU)
Programme holder Institut Bauen und Umwelt e.V. (IBU)
Declaration number EPD-STO-20230192-CBA1-EN
Issue date 11.08.2023
Valid to 10.08.2028
StoVentec Glass A
Sto SE & Co. KGaA
www.ibu-epd.com | https://epd-online.com
General Information
Sto SE & Co. KGaA StoVentec Glass A
Programme holder Owner of the declaration
IBU – Institut Bauen und Umwelt e.V. Sto Scandinavia AB
Hegelplatz 1 Gesällgatan 6
10117 Berlin 58110 Linköping
Germany Sweden
Declaration number Declared product / declared unit
EPD-STO-20230192-CBA1-EN 1m² of the product StoVentec Glass A (incl. Sto-Agrafe Profile).
This declaration is based on the product category rules: Scope:
Curtain walling, 01.08.2021 This environmental product declaration does only include the StoVentec
(PCR checked and approved by the SVR) Glass A panel itself as well as the agrafe profile fixed to the
subconstruction / wall but not the insulation and not the subconstruction
being used within the Rainscreen Cladding system.
Issue date
Within this environmental product declaration the specific product named
11.08.2023
"StoVentec Glass A" with a fire behaviour classification A2-s1,d0 in
accordance with EN 13501-1 is described.
Valid to
Environmental data of the product named "StoVentec Glass" with a fire
10.08.2028 behaviour classification B-s1,d0 in accordance with EN 13501-1 can be
found in the annexe.
Product components are produced by Sto SE & Co. KGaA (production
sites at Lauingen, Germany) and by external suppliers.
The owner of the declaration shall be liable for the underlying information
and evidence; the IBU shall not be liable with respect to manufacturer
information, life cycle assessment data and evidences.
The EPD was created according to the specifications of EN 15804+A2. In
the following, the standard will be simplified as EN 15804.
Verification
Dipl.-Ing. Hans Peters
(Chairman of Institut Bauen und Umwelt e.V.) The standard EN 15804 serves as the core PCR
Independent verification of the declaration and data according to ISO
14025:2011
internally X externally
Florian Pronold Matthias Schulz,
(Managing Director Institut Bauen und Umwelt e.V.) (Independent verifier)
1 Environmental Product Declaration - Sto SE & Co. KGaA - StoVentec Glass A
Product
Other constructional data are not relevant.
Product description/Product definition
The StoVentec Glass A product is a composite panel Performance data of the product with respect to its
comprising a toughened enamelled glass which is bonded to a characteristics in accordance with the relevant technical
lightweight carrier board (made of expanded perlite granulate) provision (no CE-marking).
with an integrated panel carrier profile on the back side. The
panel itself is being used within Rainscreen Cladding systems Base materials/Ancillary materials
with a joint-accentuated appearance. The StoVentec Glass A panel (incl. Sto-Agrafe Profile) has a
total mass of around 29,1 kg/m2 comprising the following
The StoVentec Glass A product offers a wide range of different components:
design options regarding formats, colours, glass types as well
as glass surfaces. Thanks to the prefabrication of the panels,
• 6 mm toughened Glass (<60% by mass)
the installation on site is easy and not depending on weather
• Silicone- based adhesive (<2% by mass)
conditions.
• 15 mm Verolith Carrier Board (<35% by mass)
For the placing of the product on the market in the European
• Sto-Board Carrier Profile (<10% by mass)
Union/European Free Trade Association/EU/EFTA (with the
• Sto-Agrafe Profile (<10% by mass)
exception of Switzerland) the Regulation (EU) No. 305/2011
(CPR) applies. The product needs a declaration of performance
This product/article/at least one partial article contains
taking into consideration ETA-23/0283 of 2023/05/15 StoVentec
substances listed in the
Glass A and the CE marking.
candidate list (date: 17.01.2023) exceeding 0.1 percentage by
mass:
For the application and use the respective national provisions
No.
apply.
For example in Germany the "Allgemeine bauaufsichtliche
This product/article/at least one partial article does contain
Zulassung Z-10.3-720", issued by the Deutsches Institut für
other carcinogenic, mutagenic, reprotoxic (CMR) substances in
Bautechnik (DiBt) Berlin, applies.
categories 1A or 1B which are not on the candidate list,
exceeding 0.1 percentage by mass: No.
Application
The declared product StoVentec Glass A is being used as a
Biocide products were added to this construction product or it
joint-accentuated facade panel within an RSC (Rainscreen
has been treated with biocide products (this then concerns a
cladding) system. For the application and use national
treated product as defined by the (EU) Ordinance on Biocide
regulations
Products No.
apply.
528/2012): No.
Technical Data
Reference service life
StoVentec Glass A Panel
With regular installation and proper maintenance, the system
Name Value Unit
can reach the life span of the building. A reference service life
max. according to ISO 15686 is not reported.
Formats vertical m
1,25x4,5
max. Maintenance
Formats horizontal m
3,75x1,5 The surface quality is affected by climatic and
Panel Weight (depending on glass environmental influences on the system over time.
27 kg/m²
thickness 6)
Panel thickness (without backrail) 23 mm
Fire resistance class acc. EN 13501-1 A2-s1,d0 class
LCA: Calculation rules
Declared Unit Production Stage (A1-A3): The Product stage includes:
The declared unit for the StoVentec Glass A facade system is 1
• A1 Raw material supply and processing,
m².
• A2 Transport of raw materials to the manufacturer,
Declared unit • A3 Production of StoVentec Glass A in the factory, (incl.
Name Value Unit energy provision, water provision, production of
Declared unit 1 m2 packaging materials)
Grammage (with agraffenprofiles ) 29.1 kg/m2
Layer thickness (without agraffenprofiles) 0.023 m Construction stage (A4-A5): The construction process stage
Layer thickness (with agraffenprofiles ) 0.055 m includes:
• A4 transport to the construction site 100km by truck,
System boundary • A5 installation of the product with a machine and
Type of EPD: Cradle to gate with options, modules C1- C4 and treatment of the packaging materials in waste
module D (A1-A3 + C + D and additional modules: A4, A5). The incineration units after installation of the product
LCA considers the following modules of the life cycle:
2 Environmental Product Declaration - Sto SE & Co. KGaA - StoVentec Glass A
End-of-life stage (C1-C4): The end-of-life stage includes:
Geographic Representativeness
• C1 de-construction with machine
Land or region, in which the declared product system is
• C2 transport to waste processing; 50 km with truck
manufactured, used or handled at the end of the product´s
Transport distance can be adjusted at building level if
lifespan: Europe
necessary (e.g., for 100 km actual transport distance:
multiply LCA values by factor 2).
• C4 disposal of the product in a landfill for inert matter Comparability
Basically, a comparison or an evaluation of EPD data is only
possible if all the data sets to be compared were created
Benefits and loads beyond the System Boundary (D):
according to EN 15804 and the building context, respectively
Module D includes:
the product-specific characteristics of performance, are taken
Loads and benefits from material recycling of metals and
into account.
energy recovery potentials from the thermal treatment of the
The background data comes from the GaBi database
pallets and mixed plastic waste from packaging.
GaBi software Version CUP2022.2
LCA: Scenarios and additional technical information
Characteristic product properties of biogenic carbon
End of life (C1-C4)
Deconstruction (C1)
Information on describing the biogenic Carbon Content at The product dismantling from the building is done with a
factory gate machine
Name ValueUnit
kg Transport to EoL treatment (C2)
Biogenic carbon content in product -
C Transport to waste treatment: 50 km by truck
Biogenic carbon content in accompanying kg
0.795 Disposal (C4)
packaging C
landfilling
Name Value Unit
Recycling 3.8 kg
Landfilling 25.3 kg
Transport from the gate to the site (A4) Reuse, recovery and/or recycling potentials (D), relevant
Name Value Unit scenario information
Transport distance 100 km European datasets have been used.
Name Value Unit
Assembly (A5)
For energy recovery (packaging) 2.5 kg
Module A5 includes installation of the product with a machine
and the treatment and disposal of packaging material. Benefits
for potential avoided burdens due to energy substitution of
electricity and thermal energy generation are declared in
module D and affects only the rate of
primary material (no secondary materials)
Name Value Unit
Electricity consumption 0.2362 MJ/m²
wooden pallets 2.04 kg/m²
polyethylene 0.03 kg/m²
polystyrene 0.34 kg/m²
polypropylene 0.09 kg/m²
3 Environmental Product Declaration - Sto SE & Co. KGaA - StoVentec Glass A
LCA: Results
DESCRIPTION OF THE SYSTEM BOUNDARY (X = INCLUDED IN LCA; ND = MODULE OR INDICATOR NOT DECLARED; MNR =
MODULE NOT RELEVANT)
Benefits and
Construction loads beyond
Product stage Use stage End of life stage
process stage the system
boundaries
la ire ta m w a Ry lp p u s tro p s n a rT g n iru tc a fu n a M e h t m o rf tro p s n a rTe tis e h t o t e ta g y lb m e s s A e s U e c n a n e tn ia M ria p e R tn e m e c a lp e R tn e m h s ib ru fe R y g re n e la n o ita re p Oe s u re ta w la n o ita re p Oe s u n o itc u rts n o c -e Dn o itilo m e d tro p s n a rT g n is s e c o rp e ts a W la s o p s iD -e s u e R-y re v o c e R-g n ilc y c e Rla itn e to p
A1 A2 A3 A4 A5 B1 B2 B3 B4 B5 B6 B7 C1 C2 C3 C4 D
X X X X X MND MND MNR MNR MNR MND MND X X X X X
RESULTS OF THE LCA - ENVIRONMENTAL IMPACT according to EN 15804+A2: 1 m² StoVentec Glass A ventilated facade
system
Parameter Unit A1-A3 A4 A5 C1 C2 C3 C4 D
GWP-total kg CO 2 eq 7.13E+01 2.08E-01 5.26E+00 2.75E-02 1.04E-01 0 3.78E-01 -2.96E+01
GWP-fossil kg CO 2 eq 7.41E+01 2.07E-01 1.6E+00 2.75E-02 1.04E-01 0 3.78E-01 -2.95E+01
GWP-biogenic kg CO 2 eq -2.88E+00 0 3.66E+00 1.62E-05 0 0 0 -7.89E-02
GWP-luluc kg CO 2 eq 3.43E-02 1.15E-03 1.03E-05 1.78E-06 5.75E-04 0 6.97E-04 -5.2E-03
ODP kg CFC11 eq 1.22E-10 1.24E-14 6.1E-13 2.72E-13 6.18E-15 0 8.87E-13 -3.04E-11
AP mol H+ eq 3.78E-01 1.97E-04 7E-04 4.04E-05 9.84E-05 0 2.68E-03 -1.44E-01
EP-freshwater kg P eq 7.62E-05 6.16E-07 9.28E-08 1.23E-08 3.08E-07 0 6.4E-07 -1.29E-05
EP-marine kg N eq 7.17E-02 6.13E-05 2.12E-04 1.1E-05 3.07E-05 0 6.84E-04 -1.71E-02
EP-terrestrial mol N eq 8.06E-01 7.37E-04 3.25E-03 1.18E-04 3.69E-04 0 7.52E-03 -1.86E-01
kg NMVOC
POCP 1.86E-01 1.71E-04 5.83E-04 3.12E-05 8.57E-05 0 2.08E-03 -5.36E-02
eq
ADPE kg Sb eq 3.89E-04 1.72E-08 1.15E-08 3.27E-09 8.62E-09 0 3.87E-08 -2.17E-06
ADPF MJ 1.02E+03 2.76E+00 1.52E+00 5.83E-01 1.38E+00 0 4.95E+00 -3.76E+02
m3 world eq
WDP 7.66E+00 1.85E-03 5.12E-01 2.05E-03 9.25E-04 0 4.14E-02 -4.63E+00
deprived
GWP = Global warming potential; ODP = Depletion potential of the stratospheric ozone layer; AP = Acidification potential of land and water; EP =
Eutrophication potential; POCP = Formation potential of tropospheric ozone photochemical oxidants; ADPE = Abiotic depletion potential for non-fossil
resources; ADPF = Abiotic depletion potential for fossil resources; WDP = Water (user) deprivation potential)
RESULTS OF THE LCA - INDICATORS TO DESCRIBE RESOURCE USE according to EN 15804+A2: 1 m² StoVentec Glass A
ventilated facade system
Parameter Unit A1-A3 A4 A5 C1 C2 C3 C4 D
PERE MJ 2.71E+02 1.57E-01 2.23E+01 8.43E-02 7.83E-02 0 7.42E-01 -1.78E+02
PERM MJ 2.2E+01 0 -2.2E+01 0 0 0 0 0
PERT MJ 2.93E+02 1.57E-01 3.01E-01 8.43E-02 7.83E-02 0 7.42E-01 -1.78E+02
PENRE MJ 9.85E+02 2.76E+00 1.97E+01 5.83E-01 1.38E+00 0 2.67E+01 -3.77E+02
PENRM MJ 3.99E+01 0 -1.82E+01 0 0 0 -2.17E+01 0
PENRT MJ 1.02E+03 2.76E+00 1.52E+00 5.83E-01 1.38E+00 0 4.95E+00 -3.77E+02
SM kg 0 0 0 0 0 0 0 3.61E+00
RSF MJ 0 0 0 0 0 0 0 0
NRSF MJ 0 0 0 0 0 0 0 0
FW m3 5.73E-01 1.77E-04 1.21E-02 1.28E-04 8.86E-05 0 1.26E-03 -4.41E-01
PERE = Use of renewable primary energy excluding renewable primary energy resources used as raw materials; PERM = Use of renewable primary
energy resources used as raw materials; PERT = Total use of renewable primary energy resources; PENRE = Use of non-renewable primary energy
excluding non-renewable primary energy resources used as raw materials; PENRM = Use of non-renewable primary energy resources used as raw
materials; PENRT = Total use of non-renewable primary energy resources; SM = Use of secondary material; RSF = Use of renewable secondary fuels;
NRSF = Use of non-renewable secondary fuels; FW = Use of net fresh water
RESULTS OF THE LCA – WASTE CATEGORIES AND OUTPUT FLOWS according to EN 15804+A2:
1 m² StoVentec Glass A ventilated facade system
Parameter Unit A1-A3 A4 A5 C1 C2 C3 C4 D
HWD kg 9.39E-08 1.32E-11 1.31E-10 4.17E-11 6.61E-12 0 2.54E-10 4.12E-08
NHWD kg 1.33E+01 3.96E-04 3.23E-02 1.24E-04 1.98E-04 0 2.53E+01 -8.18E+00
RWD kg 3.99E-02 3.4E-06 1.52E-04 9.69E-05 1.7E-06 0 5.51E-05 -2.39E-02
CRU kg 0 0 0 0 0 0 0 0
MFR kg 0 0 0 3.8E+00 0 0 0 0
MER kg 0 0 0 0 0 0 0 0
4 Environmental Product Declaration - Sto SE & Co. KGaA - StoVentec Glass A
EEE MJ 0 0 8.2E+00 0 0 0 0 0
EET MJ 0 0 1.47E+01 0 0 0 0 0
HWD = Hazardous waste disposed; NHWD = Non-hazardous waste disposed; RWD = Radioactive waste disposed; CRU = Components for re-use;
MFR = Materials for recycling; MER = Materials for energy recovery; EEE = Exported electrical energy; EET = Exported thermal energy
RESULTS OF THE LCA – additional impact categories according to EN 15804+A2-optional:
1 m² StoVentec Glass A ventilated facade system
Parameter Unit A1-A3 A4 A5 C1 C2 C3 C4 D
Disease
PM 3.35E-06 1.19E-09 3.73E-09 3.61E-10 5.93E-10 0 3.29E-08 -1.5E-06
incidence
IR kBq U235 eq 7.35E+00 4.99E-04 2.33E-02 1.42E-02 2.49E-04 0 6.12E-03 -4.97E+00
ETP-fw CTUe 7.86E+02 1.91E+00 5.93E-01 1.79E-01 9.57E-01 0 2.77E+00 -1.34E+02
HTP-c CTUh 3.65E-08 3.86E-11 3.49E-11 3.29E-12 1.93E-11 0 4.23E-10 -1.72E-08
HTP-nc CTUh 2.15E-06 2.01E-09 1.25E-09 1.7E-10 1.01E-09 0 4.69E-08 -3.6E-07
SQP SQP 6.08E+02 9.48E-01 3.31E-01 5.35E-02 4.74E-01 0 1.03E+00 -1.6E+01
PM = Potential incidence of disease due to PM emissions; IR = Potential Human exposure efficiency relative to U235; ETP-fw = Potential comparative
Toxic Unit for ecosystems; HTP-c = Potential comparative Toxic Unit for humans (cancerogenic); HTP-nc = Potential comparative Toxic Unit for humans
(not cancerogenic); SQP = Potential soil quality index
Disclaimer 1 – for the indicator “Potential Human exposure efficiency relative to U235”. This impact category deals mainly with the
eventual impact of low-dose ionizing radiation on human health of the nuclear fuel cycle. It does not consider effects due to possible
nuclear accidents, occupational exposure or radioactive waste disposal in underground facilities. Potential ionizing radiation from the
soil, radon and from some construction materials is also not measured by this indicator.
Disclaimer 2 – for the indicators “abiotic depletion potential for non-fossil resources”, “abiotic depletion potential for fossil resources”,
“water (user) deprivation potential, deprivation-weighted water consumption”, “potential comparative toxic unit for ecosystems”,
“potential comparative toxic unit for humans – cancerogenic”, “Potential comparative toxic unit for humans - not cancerogenic”,
“potential soil quality index”. The results of this environmental impact indicator shall be used with care as the uncertainties on these
results are high as there is limited experience with the indicator.
References
Standards EN 15804
EN 15804:2012-04+A1 2013, Sustainability of construction
AbZ: Z-10.3-720 works — Environmental Product Declarations — Core rules for
National technical approval Z-10.3-720 Includes "StoVentec the product category of construction products.
Glass" panels for use in rainscreen cladding façade or ceiling
coverings, issued by the Deutsches Institut für Bautechnik ISO 14025
(DiBt), Berlin DIN EN ISO 14025:2011-10, Environmental labels and
declarations — Type III environmental declarations —
EAD 090019-00-0404 Principles and procedures.
Kits for ventilated external wall claddings of lightweight boards
on subframe with rendering applied in situ with or without ISO 15686
thermal insulation. Buildings and constructed assets - Service life planning.
DIN EN 410 Further References
The DIN EN 410 specifies the calculation method for
determining the photometric and BBSR
radiation-physical parameters of glazing. Service Life of Building Components; version 03.11.2011:
https://www.nachhaltigesbauen.de/austausch/nutzungsdauern-
DIN EN 12154 von-bauteilen/.
DIN EN 12154:2000-06, Curtain walling - Watertightness -
Performance requirements Candidate list
and classification. Candidate list of substances of very high concern for
Authorisation - published in accordance
DIN EN 13363-1 with Article 59(10) of the REACH Regulation.
Solar protection devices combined with glazing - Calculation of
solar and light transmittance - Part 1: Simplified method GaBi ts documentation
GaBi life cycle inventory data documentation
DIN EN 13363-2 (https://www.gabisoftware.com/support/gabi/gabidatabase2020lcidocumentation/)
Solar protection devices combined with glazing - Calculation of
total solar energy transmittance and light transmittance - Part 2: GaBi ts software
Detailed calculation method Sphera Solutions GmbH
GaBi Software System and Database for Life Cycle
DIN EN 13501 Engineering
DIN EN 13501-1:2019-05:Fire classification of construction CUP Version: 2022.2
products and building elements – Part 1: Classification using University of Stuttgart
data from reaction to fire tests; German version EN 13501- Leinfelden Echterdingen
1:2018.
5 Environmental Product Declaration - Sto SE & Co. KGaA - StoVentec Glass A
IBU 2021 PCR Part A
Institut Bauen und Umwelt e.V.: General Programme PCR - Part A: Calculation Rules for the Life CycleAssessment
Instructions for the Preparation of EPDs at the Institut Bauen and Requirements on the Project
und Umwelt e.V. Version 2.0, Berlin: Institut Bauen und Umwelt Report,Berlin: Institut Bauen und Umwelt e.V., www.ibu-
e.V., 2021 epd.com, Version 1.3, 2021
Lengsfeld 2015 PCR B: Curtain Walling
Lengsfeld, Kristin: Beurteilung der Langzeitbewährung von PCR Guidance-Texts for Building-Related Products and
Ausgeführten Services. Part B: Requirements on the EPD for Curtain walling,
Wärmedämmverbundsystemen, Fraunhofer IBP-Bericht HTB- Version 1. Berlin: Institut Bauen und Umwelt e.V. (Ed.), 2023.
06/2015, beauftragt vom
Fachverband Wärmedämmverbundsystem e. V., Juni 2015.
6 Environmental Product Declaration - Sto SE & Co. KGaA - StoVentec Glass A
Publisher
Institut Bauen und Umwelt e.V. +49 (0)30 3087748- 0
Hegelplatz 1 info@ibu-epd.com
10117 Berlin www.ibu-epd.com
Germany
Programme holder
Institut Bauen und Umwelt e.V. +49 (0)30 3087748- 0
Hegelplatz 1 info@ibu-epd.com
10117 Berlin www.ibu-epd.com
Germany
Author of the Life Cycle Assessment
Sphera Solutions GmbH +49 711 341817-0
Hauptstraße 111- 113 info@sphera.com
70771 Leinfelden-Echterdingen www.sphera.com
Germany
Owner of the Declaration
Sto Scandinavia AB +46 13 37 71 00
Gesällgatan 6 kundkontakt@sto.com
58110 Linköping www.sto.se
Sweden
Sto SE & Co. KGaA +49 7744 57-1010
Ehrenbachstr. 1 infoservice@sto.com
79780 Stühlingen www.sto.com
Germany
7 Environmental Product Declaration - Sto SE & Co. KGaA - StoVentec Glass A
