ENVIRONMENTAL PRODUCT DECLARATION
as per ISO 14025 and EN 15804+A2
Owner of the Declaration STS
Publisher Institut Bauen und Umwelt e.V. (IBU)
Programme holder Institut Bauen und Umwelt e.V. (IBU)
Declaration number EPD-SHA-20230445-CBA6-EN
Issue date 18.12.2023
Valid to 17.12.2028
STS Carpet Tile with Nylon Face Fibre
STS (Sanquhar Tile Services) (Shaw Europe
Ltd.)
www.ibu-epd.com | https://epd-online.com
General Information
STS (Sanquhar Tile Services) (Shaw Europe STS Carpet Tile with Nylon Face Fibre
Ltd.)
Programme holder Owner of the declaration
IBU – Institut Bauen und Umwelt e.V. STS
Hegelplatz 1 Blackaddie Road *
10117 Berlin DG46DB Sanquhar
Germany United Kingdom
Declaration number Declared product / declared unit
EPD-SHA-20230445-CBA6-EN 1 m2 of installed STS Bitumen Backed Carpet Tile
This declaration is based on the product category rules: Scope:
Floor coverings, 01.08.2021 A Life Cycle Assessment (LCA) was conducted based upon production
(PCR checked and approved by the SVR) data collected from STS, Plant SQ manufacturing facility (Blackaddie
Road, Sanquhar, DG46DB), located in Scotland, UK. Production data was
collected for STS Premium Loop Pile Tufted, Bitumen Backed Carpet Tile
Issue date with Nylon Face Fibre, for the period of one year, from January to
December 2021.
18.12.2023
This EPD is cradle-to-gate with options in scope with additional modules
A4, A5, B1 and B2. The EPD is created in accordance to the specifications
Valid to
of EN 15804+A2.
17.12.2028
The functional unit has been defined as 1 m2 of installed STS Premium
Loop Pile Tufted, Bitumen Backed Carpet Tile.
The EPD was generated with the help of Envision LCA Tool, version 1. The
tool has not been manipulated in calculating impact results. The current
version of the tool is maintained, saved, and stored for 10 years to be used
for revision and re-traceability purposes.
The owner of the declaration shall be liable for the underlying information
and evidence; the IBU shall not be liable with respect to manufacturer
information, life cycle assessment data and evidences.
Dipl.-Ing. Hans Peters The EPD was created according to the specifications of EN 15804+A2. In
(Chairman of Institut Bauen und Umwelt e.V.) the following, the standard will be simplified as EN 15804.
Verification
The standard EN 15804 serves as the core PCR
Independent verification of the declaration and data according to ISO
14025:2011
internally X externally
Florian Pronold Mrs Kim Allbury,
(Managing Director Institut Bauen und Umwelt e.V.) (Independent verifier)
1 Environmental Product Declaration - STS (Sanquhar Tile Services) (Shaw Europe Ltd.) - STS Carpet Tile with Nylon Face Fibre
Product
Name Value Unit
Product description/Product definition
Product thickness 5.8 - 6.2 mm
This EPD applies to STS Premium Loop Pile Tufted, Bitumen
Backed Carpet Tile with Nylon face fibre.
Grammage 3896.4 g/m2
Product Form Carpet Tile -
The carpet tile backing system contains a modified bitumen Yarn type - Solution-dyed 0% Post-industrial
-
polymer, mineral filler, and a fibreglass reinforcement layer for Nylon 6 Recycled Content
dimensional stability. The face fibre is made of solution-dyed
Total thickness 5.8 - 6.2 mm
Nylon that is tufted into a primary backing sheet, then latex is
Total carpet weight 3600 - 4170 g/m2
added to anchor the fibre in place to assure maximum tuft bind.
The bitumen-based backing system is then applied to create a Surface pile thickness 2.4 - 2.6 mm
durable flooring solution for use in varied applications. The Surface pile weight - Nominal
610 - 800 g/m2
carpet tiles are then die-cut and packaged for distribution. Pile Mass
Length and width of squared
250 - 1000 mm
This STS Premium Loop Pile Tufted, Bitumen Backed Carpet elements
Tile is a commercial carpet tile, suitable for use in all
Other technical data parameters listed in IBU PCR Part B are
commercial settings as a floor covering, in accordance with
not relevant and, therefore, have not been declared.
manufacturer guidelines. It has a life span of 10 years and
comes with a 10-year wear warranty (subject only to installation
Performance data of the product in accordance with the
and maintenance being carried out in line with manufacturer's
declaration of performance with respect to its essential
guidelines). The product meets both internal and external
characteristics according to 14041:2004A/C:2006.
performance standards including those established in the EU
under EN 1307 and EN 10874 for a product suitable for heavy
Base materials/Ancillary materials
and general commercial installations.
STS Premium Loop Pile Tufted, Bitumen Backed Carpet Tile
with Nylon Face Fibre is comprised of the following raw
STS Premium Loop Pile Tufted, Bitumen Backed Carpet Tile
materials:
comes in various styles. All styles have the same raw material
formulation but different designs. • 50-60% Calcium Carbonate Filler
• 12-18% Modified Bitumen Polymer
This product is manufactured in the UK in ISO 9001- and ISO • 12-18% Solution-dyed Nylon 6 Face Fibre
14001-certified facilities, or equivalent. Raw materials are • 8-13% Styrene Butadiene Co-Polymer Latex
responsibly sourced through supply chain, chemical and waste • 1-4% Polyester Primary Backing
management programs. No co-products are produced in the • 1-3% Polypropylene Secondary Backing
manufacturing of these premium carpet tiles. • 0.1-1% Fibreglass Reinforcement
• 0-0.1% Anti-stat
Detailed Product Descriptions: The product is packaged in cardboard boxes, wrapped in
For the application and use, the respective national provisions plastic, and stacked on wooden pallets for distribution.
apply.
The product fits into the defined scope and all raw material
Application inputs, with no exceptions, are captured by the Envision LCA
STS Premium Loop Pile Tufted, Bitumen Backed Carpet Tile Tool, version 1.
with Nylon Face Fibre is suitable for use as a floor covering in
heavy and general commercial installations. This product contains substances listed in the candidate list
(date: 17.01.2023) exceeding 0.1 percentage by mass: no
Technical Data
The technical specifications of the product are listed on the This product contains other CMR substances in categories 1A
product's specification sheet, found at or 1B which are not on the candidate list, exceeding 0.1
STSorders@sanquhartilesltd.co.uk. This product meets the percentage by mass: no
requirements of the harmonized European Norm (hEN):
EN14041:2004A/C:2006. Declarations of performance related Biocide products were added to this construction product or it
to fire, electrostatic, formaldehyde emissions, and slip has been treated with biocide products (this then concerns a
resistance can be found on the product's specification sheet. treated product as defined by the (EU) Ordinance on Biocide
Constructional data Products No. 528/2012): no
Reference service life
When properly installed as a commercial floor covering, STS
Premium Loop Pile Tufted, Bitumen Backed Carpet Tile with
Nylon face fibre has a reference service life of 10 years. This
carpet tile product comes with a 10-year warranty, subject only
to installation and maintenance being carried out in accordance
with the manufacturer's guidelines.
LCA: Calculation rules
The declaration refers to the declared unit of 1 m² of installed
Declared Unit carpet tile.
Declared unit
2 Environmental Product Declaration - STS (Sanquhar Tile Services) (Shaw Europe Ltd.) - STS Carpet Tile with Nylon Face Fibre
Name Value Unit • Module B6 - Operational Energy Use (module not
Declared unit 1 m2 relevant).
• Module B7 - Operational Water Use (module not
Grammage 3.896 kg/m2
relevant).
Layer thickness 0.006 m End of Life Stage:
Three scenarios have been evaluated:
System boundary Scenario 1: the STS Bitumen Backed carpet is 100% disposed
The type of EPD is Cradle-to-Gate with options modules C1– of in a landfill.
C4, module D, and additional modules. The additional modules Scenario 2: the STS Bitumen Backed carpet is 100%
are A4, A5, B1 and B2. incinerated.
Scenario 3: 40% of STS Bitumen Backed carpets are
The modules considered in the life cycle assessment and incinerated and the remaining 60% are landfilled. This
environmental product declaration, based on the product's assumption is based on the carpet disposal rates in Europe
entire life cycle, are described as follows: mentioned in the study conducted by Deutsche Umwelthilfe in
2017 (Umwelthilfe, 2017) and the European Commission in
Production Stage: 2013 (Commission, 2013).
• Module A1 - Provision of Raw Materials. • Module C1 - The carpet is de-constructed manually and
• Module A2 - Transport of Raw Materials. no additional environmental impact is caused.
• Module A3 - Manufacturing. • Module C2 - Transport of the carpet waste to a landfill or
Construction/Installation Stage: to the municipal waste incineration plant.
• Module C3 - Impacts from thermal treatment disposal
• Module A4 - Transportation by truck of the product to the
(C3/2 and C3/3).
construction site in Europe.
• Module C4 - Impacts from landfill disposal (C4/1 and
• Module A5 - Installation of the carpet, treatment of
C4/3).
cutting waste (landfill) and packaging waste (landfill,
Module D includes benefits from energy recovery via treatment
recycling, and incineration). The production of the
of packaging materials and incineration of carpets at their end
amount of carpet that occurs as installation waste is
of life (D/1, D/2 and D/3), as well as the burdens of balancing
also included along with its transport to the place of
the secondary material content in modules A1 and A3 via the
installation. Biogenic carbon that is stored in the wooden
net-scrap approach.
pallets and cardboard (packaging) is released as carbon
dioxide emissions into the air at the end of life in module Geographic Representativeness
A5.
Land or region, in which the declared product system is
Use Stage:
manufactured, used or handled at the end of the product´s
• Module B1 - Indoor emissions of volatile organic lifespan: Europe
compounds (VOCs) during the first few months after
installation.
Comparability
• Module B2 - Carpet cleaning per year, including
vacuuming (electricity consumption) and hot water Basically, a comparison or an evaluation of EPD data is only
cleaning (electricity and water consumption, as well as possible if all the data sets to be compared were created
waste water treatment). according to EN 15804 and the building context, respectively
• Module B3 - Repair (module not relevant). the product-specific characteristics of performance, are taken
• Module B4 - Replacement (module not relevant). into account. The background database used for the creation of
• Module B5 - Refurbishment (module not relevant). the EPD: GaBi ts software, CUP 2022.2.
LCA: Scenarios and additional technical information
adhesive is required for the installation of STS Bitumen Backed
Characteristic product properties of biogenic carbon Carpet Tile and should be used in accordance with the
Biogenic carbon is only present in packaging (wooden pallets manufacturer's guidelines. Installation losses have been
and cardboards). Assumed water content in wooden pallet accounted for in module A5. Product losses are considered as
(packaging): 18%. 5%.
Information on describing the Biogenic Carbon Content at
factory gate The packaging material treatment and disposal are also
considered in module A5 (landfill, recycling, and incineration)
Name ValueUnit
and the resulting benefits from energy generation are included
Biogenic carbon content in accompanying kg
0.14 in module D. The quantity of wooden pallets used is 0.133 kg
packaging C
per m². Wooden pallets are assumed to be re-used 20 times
before being disposed of. Hence, the quantity of pallet disposed
The following technical scenario information is required for the is 0.007 kg. The quantity of cardboard packaging is 0.21 kg/m²
declared modules and optional for non-declared modules. and the quantity of plastic packaging is 0.0103 kg/m². Total
amount of packaging disposed at installation is 0.227 kg.
Transport to the construction site (A4)
Packaging disposal rates (Source: Eurostat, Recovery and
Name Value Unit recycling rates for packaging).
Transport distance (truck) 687 km
• Paper - 82.8% recycled; 9.4% landfilled; and 7.8%
Capacity utilisation (including empty runs) 55 % incinerated
• Plastic - 40.3% recycled; 28.7% landfilled; and 31.0%
Installation in the building (A5)
incinerated
The installation of STS Bitumen Backed Carpet Tile is done • Wood pallets - 39.8% recycled; 34.5% landfilled; and
manually and no energy is required. A Pressure-Sensitive 25.7% incinerated
3 Environmental Product Declaration - STS (Sanquhar Tile Services) (Shaw Europe Ltd.) - STS Carpet Tile with Nylon Face Fibre
Name ValueUnit C2 - Transportation of the product to the end of life is assumed
to be 161 km (100 miles).
Auxiliary 0.23 kg
C3/2 - The STS Bitumen Backed carpet is 100% combusted in
Material loss 0.203 kg
an incineration plant with energy recovery (R>0.6).
Output substances following waste treatment on
0.227 kg C3/3 - It is assumed that 40% of STS Bitumen Backed carpets
site (packaging materials)
are incinerated and the remaining 60% are landfilled.
C4/1 - The STS Bitumen Backed carpet is 100% disposed of in
Maintenance (B2)
landfill.
For the maintenance of STS Bitumen Backed Carpet Tile, 2 hot
C4/3 - It is assumed that 40% of STS Bitumen Backed carpets
water extraction cleanings (water and electricity consumption)
are incinerated and the remaining 60% are landfilled.
per year as well as 52 vacuum cleanings (electricity
Name ValueUnit
consumption) per year are recommended. The Reference
Service Life of the product is 10 years. The results in the EPD Collected as mixed construction waste 3.896 kg
declare a maintenance for the period of 1 year. Landfilling (Scenario 1 - C3/1, C4/1 and D/1) 3.896 kg
Name Value Unit Incineration (Scenario 2 - C3/2, C4/2, and D/2) 3.896 kg
Water consumption (1 year) 0.0009 m3 Landfilling (60%) and Incineration (40%) (Scenario
3.896 kg
3 - C3/3, C4/3 and D/3)
Electricity consumption (1 year) 0.772 kWh
Reference service life Reuse, recovery and/or recycling potentials (D), relevant
Name ValueUnit scenario information
Reference service life (according to ISO 15686-1, - For the thermal and electrical energy generated in Module A5
12 a
2, -7 and -8) due to thermal treatment of packaging, avoided burdens have
been calculated by the inversion of electricity grid mix and
Life Span according to the manufacturer 12 a
thermal energy from natural gas, using European datasets.
End of Life (C1-C4) Module D also includes the environmental burdens linked to the
supply to secondary materials (nylon and calcium carbonate)
C1 - The product dismantling from the building is done
used in the carpet production.
manually without energy burden.
4 Environmental Product Declaration - STS (Sanquhar Tile Services) (Shaw Europe Ltd.) - STS Carpet Tile with Nylon Face Fibre
LCA: Results
The B2 module declares the maintenance (cleaning) per one year. The user of the EPD will be able to scale the results for its entire
useful life by multiplying the impact by the RSL.
The LCA results presented below applies to 100% landfilled end of life scenario.
DESCRIPTION OF THE SYSTEM BOUNDARY (X = INCLUDED IN LCA; MND = MODULE OR INDICATOR NOT DECLARED; MNR
= MODULE NOT RELEVANT)
Benefits and
Construction loads beyond
Product stage Use stage End of life stage
process stage the system
boundaries
la ire ta m w a Ry lp p u s tro p s n a rT g n iru tc a fu n a M e h t m o rf tro p s n a rTe tis e h t o t e ta g y lb m e s s A e s U e c n a n e tn ia M ria p e R tn e m e c a lp e R tn e m h s ib ru fe R y g re n e la n o ita re p Oe s u re ta w la n o ita re p Oe s u n o itc u rts n o c -e Dn o itilo m e d tro p s n a rT g n is s e c o rp e ts a W la s o p s iD -e s u e R-y re v o c e R-g n ilc y c e Rla itn e to p
A1 A2 A3 A4 A5 B1 B2 B3 B4 B5 B6 B7 C1 C2 C3 C4 D
X X X X X X X MNR MNR MNR MND MND X X X X X
RESULTS OF THE LCA - ENVIRONMENTAL IMPACT according to EN 15804+A2: 1 m² STS Bitumen Backed Carpet
Parameter Unit A1-A3 A4 A5 B1 B2 C1 C2 C3 C4 D
GWP-total kg CO 2 eq 7.58E+00 2.45E-01 5.05E-01 2.54E-04 2.32E-01 0 5.28E-02 0 2.73E-01 -1.72E-02
GWP-fossil kg CO 2 eq 7.9E+00 2.44E-01 5.08E-01 2.54E-04 2.29E-01 0 5.26E-02 0 2.76E-01 -2.11E-02
GWP-
biogenic kg CO 2 eq -3.28E-01 -3.37E-04 -3.64E-03 0 2.44E-03 0 -7.26E-05 0 -2.94E-03 3.88E-03
GWP-luluc kg CO 2 eq 3.38E-03 1.36E-03 2.87E-04 0 4.85E-05 0 2.93E-04 0 1.34E-04 -3.19E-06
ODP kg CFC11 eq 8.28E-09 1.46E-14 4.36E-10 0 3.35E-12 0 3.15E-15 0 3.71E-13 -1.22E-13
AP mol H+ eq 1.43E-02 2.51E-04 1.17E-03 0 5.03E-04 0 5.42E-05 0 8.18E-04 -3.47E-05
EP-
kg P eq 2.07E-05 7.28E-07 1.57E-05 0 1.12E-06 0 1.57E-07 0 5.15E-05 -3.08E-08
freshwater
EP-marine kg N eq 3.63E-03 8.22E-05 2.66E-04 0 1.15E-04 0 1.77E-05 0 1.81E-04 -9.64E-06
EP-terrestrial mol N eq 3.46E-02 9.79E-04 3.27E-03 0 1.18E-03 0 2.11E-04 0 1.99E-03 -1.03E-04
kg NMVOC
POCP 1.22E-02 2.21E-04 9.72E-04 1.41E-05 3.05E-04 0 4.77E-05 0 5.83E-04 -3.14E-05
eq
ADPE kg Sb eq 1.04E-06 2.04E-08 7.99E-08 0 6.24E-08 0 4.4E-09 0 1.92E-08 -3.33E-09
ADPF MJ 1.73E+02 3.26E+00 1.05E+01 0 4.15E+00 0 7.03E-01 0 3.92E+00 -5.01E-01
m3 world eq
WDP 3.57E-01 2.19E-03 8.86E-02 0 5.23E-02 0 4.72E-04 0 -2.72E-03 -2.98E-03
deprived
GWP = Global warming potential; ODP = Depletion potential of the stratospheric ozone layer; AP = Acidification potential of land and water; EP =
Eutrophication potential; POCP = Formation potential of tropospheric ozone photochemical oxidants; ADPE = Abiotic depletion potential for non-fossil
resources; ADPF = Abiotic depletion potential for fossil resources; WDP = Water (user) deprivation potential)
RESULTS OF THE LCA - INDICATORS TO DESCRIBE RESOURCE USE according to EN 15804+A2: 1 m² STS Bitumen Backed
Carpet
Parameter Unit A1-A3 A4 A5 B1 B2 C1 C2 C3 C4 D
PERE MJ 1.21E+01 1.95E-01 5.11E+00 0 2.31E+00 0 3.99E-02 0 3.22E-01 -1.29E-01
PERM MJ 5.31E+00 0 -4.19E+00 0 0 0 0 0 0 0
PERT MJ 1.74E+01 1.95E-01 9.21E-01 0 2.31E+00 0 3.99E-02 0 3.22E-01 -1.29E-01
PENRE MJ 1.31E+02 3.44E+00 1.57E+00 0 4.15E+00 0 7.04E-01 0 3.92E+00 -5.02E-01
PENRM MJ 5.1E+01 0 -3.17E-01 0 0 0 0 0 0 0
PENRT MJ 1.81E+02 3.44E+00 1.26E+00 0 4.15E+00 0 7.04E-01 0 3.92E+00 -5.02E-01
SM kg 1.1E-01 0 5.77E-03 0 0 0 0 0 0 -1.15E-01
RSF MJ 0 0 0 0 0 0 0 0 0 0
NRSF MJ 0 0 0 0 0 0 0 0 0 0
FW m3 2.36E-02 2.1E-04 9.32E-03 0 2.2E-03 0 4.52E-05 0 5.07E-05 -1.05E-04
PERE = Use of renewable primary energy excluding renewable primary energy resources used as raw materials; PERM = Use of renewable primary
energy resources used as raw materials; PERT = Total use of renewable primary energy resources; PENRE = Use of non-renewable primary energy
excluding non-renewable primary energy resources used as raw materials; PENRM = Use of non-renewable primary energy resources used as raw
materials; PENRT = Total use of non-renewable primary energy resources; SM = Use of secondary material; RSF = Use of renewable secondary fuels;
NRSF = Use of non-renewable secondary fuels; FW = Use of net fresh water
RESULTS OF THE LCA – WASTE CATEGORIES AND OUTPUT FLOWS according to EN 15804+A2:
1 m² STS Bitumen Backed Carpet
Parameter Unit A1-A3 A4 A5 B1 B2 C1 C2 C3 C4 D
HWD kg 3.92E-07 1.56E-11 2.31E-08 0 3.59E-10 0 3.37E-12 0 6.04E-10 -4.49E-11
NHWD kg 2.94E-01 4.68E-04 2.48E-01 0 3.82E-03 0 1.01E-04 0 3.88E+00 -2.01E-04
RWD kg 3.52E-03 4.02E-06 2.05E-04 0 6.64E-04 0 8.67E-07 0 4.81E-05 -2.33E-05
5 Environmental Product Declaration - STS (Sanquhar Tile Services) (Shaw Europe Ltd.) - STS Carpet Tile with Nylon Face Fibre
CRU kg 0 0 0 0 0 0 0 0 0 0
MFR kg 0 0 1.81E-01 0 0 0 0 0 0 0
MER kg 0 0 0 0 0 0 0 0 0 0
EEE MJ 0 0 6.37E-02 0 0 0 0 0 0 0
EET MJ 0 0 9.77E-02 0 0 0 0 0 0 0
HWD = Hazardous waste disposed; NHWD = Non-hazardous waste disposed; RWD = Radioactive waste disposed; CRU = Components for re-use;
MFR = Materials for recycling; MER = Materials for energy recovery; EEE = Exported electrical energy; EET = Exported thermal energy
RESULTS OF THE LCA – additional impact categories according to EN 15804+A2-optional:
1 m² STS Bitumen Backed Carpet
Parameter Unit A1-A3 A4 A5 B1 B2 C1 C2 C3 C4 D
Disease
PM 1.36E-07 1.45E-09 1.2E-08 0 4.17E-09 0 3.13E-10 0 7.87E-09 -7.87E-10
incidence
IR kBq U235 eq 3.76E-01 5.9E-04 2.24E-02 0 1.12E-01 0 1.27E-04 0 7.11E-03 -3.92E-03
ETP-fw CTUe 9.28E+01 2.26E+00 5.93E+00 1.15E-04 1.88E+00 0 4.88E-01 0 3.83E+00 -1.94E-01
HTP-c CTUh 2.64E-09 4.56E-11 1.76E-10 0 5.43E-11 0 9.83E-12 0 1.72E-10 -5.75E-12
HTP-nc CTUh 1.34E-07 2.37E-09 9.28E-09 3.07E-12 2.12E-09 0 5.1E-10 0 1.44E-08 -2.24E-10
SQP SQP 1.4E+01 1.12E+00 1.12E+01 0 1.5E+00 0 2.42E-01 0 2.82E-01 -6.47E-01
PM = Potential incidence of disease due to PM emissions; IR = Potential Human exposure efficiency relative to U235; ETP-fw = Potential comparative
Toxic Unit for ecosystems; HTP-c = Potential comparative Toxic Unit for humans (cancerogenic); HTP-nc = Potential comparative Toxic Unit for humans
(not cancerogenic); SQP = Potential soil quality index
Disclaimer 1: For the indicator 'Potential Human exposure efficiency relative to U235". This impact category deals mainly with the
eventual impact of low dose ionizing radiation on human health of the nuclear fuel cycle. It does not consider effects due to possible
nuclear accidents, occupational exposure nor due to radioactive waste disposal in underground facilities. Potential ionizing radiation
from the soil, from radon and from some construction materials is also not measured by this indicator.
Disclaimer 2: For the indicators 'Abiotic depletion potential for non-fossil resources', 'Abiotic depletion potential for fossil resources”,
“Water (user) deprivation potential", "Deprivation-weighted water consumption”, “Potential comparative toxic unit for ecosystems”,
“Potential comparative toxic unit for humans -cancerogenic”, “Potential comparative toxic unit for humans -non-carcinogenic”, “Potential
soil quality index”. The results of these environmental impact indicators shall be used with care as the uncertainties on these results are
high or as there is limited experienced with the indicators. This EPD was created using a software tool.
References
STANDARDS: ISO 15686-2:2011, Building and constructed assets — Service
life planning — Part 2: Service life prediction procedures.
EN 10874
EN 10874:2009, Resilient, textile and laminate floor coverings ISO 15686
— Classification. ISO 15686-7:2011, Building and constructed assets — Service
life planning — Part 7: Performance evaluation for feedback of
EN 1307 service life data from practice.
EN 1307:2014, Textile floor coverings — Classification.
ISO 15686
EN 14041 ISO 15686-8:2011, Building and constructed assets — Service
EN 14041:2004/AC:2006 — Resilient, textile and laminate floor life planning — Part 8: Reference service life and service life
coverings — Essential characteristics. estimation.
EN 15804 FURTHER REFERENCES:
EN 15804:2012+A2:2019/AC:2021, Sustainability of
construction works — Environmental product declarations — Candidate list
Core rules for the product category of construction products. Candidate List of substances of very high concern for
Authorisation, published on ECHA website, latest version
ISO 14025 17.01.2023 (https://echa.europa.eu/candidatelist-table).
ISO 14025:2011, Environmental labels and declarations —
Type III environmental declarations — Principles and Deutsche Umwelthilfe
procedures. Deutsche Umwelthilfe. Swept under the Carpet: The Big Waste
Problem of the Carpet Industry in Germany, 2017.
ISO 14040
ISO 14040:2006, Environmental management — Life cycle Envision LCA Tool
assessment — Principles and framework. Envision LCA Tool, 2021, Sphera Solutions GmbH, Leinfelden-
Echterdingen, with acknowledgement of LBP University of
ISO 14044 Stuttgart, version 1.
ISO 14044:2006, Environmental management — Life cycle
assessment — Requirements and guidelines. GaBi
GaBi Software System and Database for Life Cycle
ISO 15686 Engineering, 1992-2021, Sphera Solutions GmbH, Leinfelden-
ISO 15686-1:2011, Building and constructed assets — Service Echterdingen, with acknowledgement of LBP University of
life planning — Part 1: General principles and framework. Stuttgart, program version GaBi 10; database version 2021.1.
ISO 15686 GaBi documentation
6 Environmental Product Declaration - STS (Sanquhar Tile Services) (Shaw Europe Ltd.) - STS Carpet Tile with Nylon Face Fibre
GaBi dataset documentation for the software system and Umwelt e.V., 2021.
databases, LBP, University of Stuttgart and Sphera Solutions
GmbH, Leinfelden-Echterdingen, 2021 (http://www.gabi- PCR Part B
software.com/support/gabi/gabi-database-2021-lci- Product Category Rules for Building Products, Part B:
documentation/). Requirements on the EPD for floor coverings, version 1.7, 2022
(www.bau-umwelt.de).
IBU 2021
Institut Bauen und Umwelt e.V.: General Instructions for the Packaging disposal rates
EPD programme of Institut Bauen und Umwelt e.V., Version Eurostat, Recovery and recycling rates for packaging. 2015
2.0, Berlin: Institut Bauen und Umwelt e.V., 2021 (www.ibu- (http://ec.europa.eu/eurostat/web/environment/waste/main-
epd.com). tables).
The literature referred to in the Environmental Product
PCR Part A Declaration must be listed in full.Standards already fully quoted
PCR Part A: Calculation rules for the Life Cycle Assessment in the EPD do not need to be listed here again.
and Requirements on the Background Report according to EN The current version of PCR Part A and PCR Part B of the PCR
15804:2012+A2:2019/AC:2021, Version 1.3, Institut Bauen und document on which they are based must be referenced.
7 Environmental Product Declaration - STS (Sanquhar Tile Services) (Shaw Europe Ltd.) - STS Carpet Tile with Nylon Face Fibre
Publisher
Institut Bauen und Umwelt e.V. +49 (0)30 3087748- 0
Hegelplatz 1 info@ibu-epd.com
10117 Berlin www.ibu-epd.com
Germany
Programme holder
Institut Bauen und Umwelt e.V. +49 (0)30 3087748- 0
Hegelplatz 1 info@ibu-epd.com
10117 Berlin www.ibu-epd.com
Germany
Author of the Life Cycle Assessment
Sphera Solutions GmbH +49 711 341817-0
Hauptstraße 111- 113 info@sphera.com
70771 Leinfelden-Echterdingen www.sphera.com
Germany
Owner of the Declaration
STS +44 1659 50497
Blackaddie Road * STSorders@sanquhartilesltd.co.uk
DG46DB Sanquhar STSorders@sanquhartilesltd.co.uk
United Kingdom
8 Environmental Product Declaration - STS (Sanquhar Tile Services) (Shaw Europe Ltd.) - STS Carpet Tile with Nylon Face Fibre
