ENVIRONMENTAL PRODUCT DECLARATION
as per ISO 14025 and EN 15804+A2
Owner of the Declaration Interface Europe Manufacturing BV
Publisher Institut Bauen und Umwelt e.V. (IBU)
Programme holder Institut Bauen und Umwelt e.V. (IBU)
Declaration number EPD-INT-20220230-CBB3-EN
Issue date 11.05.2023
Valid to 10.05.2028
Superflor II, Needled tiles with a total pile weight of 521 g/m² and a
CQuest Bio backing
Interface
www.ibu-epd.com | https://epd-online.com
General Information
Interface Superflor II, Needled tiles with a total pile weight
of 521 g/m² and a CQuest Bio backing
Programme holder Owner of the declaration
IBU – Institut Bauen und Umwelt e.V. Interface Europe Manufacturing BV
Hegelplatz 1 Industrielaan 15
10117 Berlin 3925ZG Scherpenzeel
Germany Netherlands
Declaration number Declared product / declared unit
EPD-INT-20220230-CBB3-EN 1 m² needled modular carpet tiles with polypropylene felt covered heavy
backing and a pile material of polyamide 6, polypropylene and polyester
with 87% recycled content
This declaration is based on the product category rules: Scope:
Floor coverings, 01.08.2021 The manufacturer declaration applies to needled carpet tiles with a
(PCR checked and approved by the SVR) polypropylene felt covered heavy backing, a pile material of PA 6, PP and
PET with a maximum total pile weight of 521 g/m2. The products are
needled in Genemuiden, the Netherlands. The carpets are back coated in
Issue date Scherpenzeel.
The declaration is only valid in conjunction with a valid GUT-PRODIS
11.05.2023
license of the product.
The owner of the declaration shall be liable for the underlying information
and evidence; the IBU shall not be liable with respect to manufacturer
Valid to
information, life cycle assessment data and evidences.
10.05.2028
The EPD was created according to the specifications of EN 15804+A2. In
the following, the standard will be simplified as EN 15804.
Verification
The standard EN 15804 serves as the core PCR
Independent verification of the declaration and data according to ISO
14025:2011
internally X externally
Dipl.-Ing. Hans Peters
(Chairman of Institut Bauen und Umwelt e.V.)
Florian Pronold Prof. Dr. Birgit Grahl,
(Managing Director Institut Bauen und Umwelt e.V.) (Independent verifier)
1 Environmental Product Declaration - Interface - Superflor II, Needled tiles with a total pile weight of 521 g/m² and a CQuest Bio backing
Product
textile and laminate floor coverings - Essential characteristics.
Product description/Product definition Additional product properties in accordance with EN 1307 can
The declaration applies to needled carpet tiles having a surface be found on the Product Information System PRODIS using the
pile of mainly solution-dyed PA 6, PP and PET with a total pile PRODIS registration number of the product (www.pro-dis.info)
weight of 521 g/m2. The backing of the carpet consists of a or on the manufacturer's technical information section.
CQuest Bio heavy backing covered by a polypropylene felt. The
total recycled content of the carpet is 62%. Base materials/Ancillary materials
CQuest Bio backing system: Name Value Unit
Backing compound based on renewable wood resin, containing Polyester 12.5 %
a recycled
Polyamide 6 9.0 %
filler and glass-fleece reinforcement. For the placing on the
Polypropylene 2.5 %
market of the specific product in the European
Union/European Free Trade Association (EU/EFTA) (with the Ethylene vinyl acetate (EVA) 5.9 %
exception of Wood resin 8.1 %
Switzerland) Regulation (EU) No. 305/2011 Construction Additives 2.1 %
Product Regulation (CPR) applies. The product needs a
Limestone 59.4 %
Declaration of Performance (DoP) taking into
Glass fiber 0.5 %
consideration EN 14041:2018-05, Resilient, textile and laminate
floor coverings - Essential characteristics, and the CE-marking. The specific product covered by the EPD contains substances
The DoP of the product can be found on the listed in the ECHA candidate list (08.07.2021) exceeding
manufacturer's technical information section. For the 0.1percentage by mass: no
application and
use of the product the respective national provisions apply. This product contains other CMR substances in categories 1A
or 1B which are not on the candidate list exceeding 0.1
Application percentage by mass: no
The use class of the specific product as defined in EN 1307 can
be found in the Product Information System (PRODIS) using Biocide products were added to this construction product or it
the PRODIS registration number of the product. has been treated with biocide products (this then concerns a
treated product as defined by the (EU) Ordinance on Biocide
Technical Data
Products No. 528/2012): no
Constructional data according to EN 1307 Aluminium hydroxide is used as fire retardant.
Name Value Unit
Reference service life
Product Form Modular carpet tiles, 50 cm x 50 cm -
The service life of textile floor coverings strongly depends on
Type of the correct installation taking into account the declared use
Needled carpet -
manufacture classification and the adherence to cleaning and maintenance
Polyamide 6, polypropylene and instructions.
Yarn type -
polyester from 87% recycled material A calculation of the reference service life according to ISO
Total carpet 15686 is not possible.
weight 4045 g/m2 Alternatively, a reference service life of 15 years can be
assumed, during which the functional and visual quality is
Secondary
CQB backing with a PP felt bottom - guaranteed. This is in accordance with the product the warranty
backing
of the manufacturer. The technical service life can be
Performance data of the product in accordance with the significantly longer.
declaration of performance with respect to its essential
characteristics according to EN 14041: 2018-05, Resilient,
LCA: Calculation rules
Declared Unit System boundary
Type of EPD: Cradle-to-gate with options
Name Value Unit System boundaries of modules A, B, C, D:
Declared unit 1 m2 Modules C3, C4 and D are indicated separately for three end-
of-life scenarios:
Grammage 4.045 kg/m2
1 - landfill disposal
Layer thickness 0.0069 m 2 - municipal waste incineration
Total thickness 6.9 mm 3 - recovery in a cement plant
Gross density 586 kg/m3 A1-A3 Production:
Energysupply and production of the basic material, processing
The declared unit refers to 1 m2 produced textile floor covering. of secondary material, auxiliary material, transport of the
The output of module A5 'Assembly' is 1 m2 installed textile material to the manufacturing site, emissions, waste water
floor covering. treatment, packaging material and waste processing up to the
landfill disposal of residual waste (except radioactive waste).
Benefits for generated electricity and steam due to the
incineration of production waste are aggregated. Biogenic
2 Environmental Product Declaration - Interface - Superflor II, Needled tiles with a total pile weight of 521 g/m² and a CQuest Bio backing
carbon that is stored in renewable material (wood resin, for recycling.
renewable additives,packaging paper) is taken into account as C3 Waste processing:
well as the associated carbon dioxide uptake from the air from C3-1: Landfill disposal needs no waste processing.
which this biogenic carbon comes. C3-2: Impact from waste incineration (plant with R1 > 0.6),
A4 Transport: generated electricity and steam are listed in the result table as
Transport of the packed textile floor covering from factory gate exported energy.
to the place of installation. C3-3:
A5 Installation: Collection of the carpet waste for recovery in the cement
Installation of the textile floor covering, processing of industry,
installation waste and packaging waste up to the landfill waste processing (granulating), transport to the cement plant,
disposal of residual waste (except radioactive waste), the emissions
production of the amount of carpet that occurs as installation from the incineration.
waste including its transport to the place of C4 Disposal
installation. C4-1: Impact from landfill disposal,
Generated electricity and steam due to the incineration of C4-2: The carpet waste leaves the system in module C3-2,
waste are listed in the result table as exported energy. C4-3: The pre-processed carpet waste leaves the system in
Biogenic carbon that is stored in renewable materials in module C3-3.
installation waste and packaging paper is released as carbon
dioxide emissions into the air at the end of life in module A5. D Recycling potential:
Preparation of the floor and auxiliary materials (adhesives, Calculated benefits result from materials exclusive secondary
fixing agents, PET connectors) are beyond the system materials (net materials).
boundaries and not taken into account. D-A5: Benefits for generated energy due to incineration of
packaging and installation waste (incineration plant with R1 >
B1 Use: 0.6),
Indoor emissions during the use stage. After the first year, no D-1: Assuming that the chemically bound renewable materials
product-related Volatile Organic Compound (VOC) emissions in a landfill gas do not release landfill gas within 100 years, no
are relevant due to known VOC decay curves of the product. benefits due to landfill dosposal of carpet waste at the
B2 Maintenance: end-of-life are taken into account,
Cleaning of the textile floor covering for a period of 1 year: D-2: Benefits for generated energy due to incineration of carpet
Vacuum cleaning – electricity supply Wet cleaning – electricity, waste at the end-of-life (incineration plant with R1 > 0.6),
water consumption, production of the cleaning agent, waste D-3: Benefits for saved fossil energy and saved inorganic
water treatment the declared values in this module have to be material due to recovery of the carpet in a cement plant.
multiplied by the assumed service life of the floor covering in
the building in question. Geographic Representativeness
B3 - B5: Land or region, in which the declared product system is
The modules are not relevant within the assumed reference manufactured, used or handled at the end of the product´s
service life of 15 years. lifespan: Europe
B6 - B7:
No energy and water input are required for the operation of the
Comparability
carpet in the use stage. The modules do not cause any
Basically, a comparison or an evaluation of EPD data is only
environmental impact.
possible if all the data sets to be compared were created
according to EN 15804 and the building context, respectively
C1 De-construction:
the product-specific characteristics of performance, are taken
The floor covering is de-constructed manually and no additional
into account. Background data are taken from the GaBi
environmental impact is caused.
database, 2022-1. Remaining data gaps are covered by the
C2 Transport:
ecoinvent 3.7 database, 2020
Transport of the carpet waste to a landfill, to the municipal
waste incineration plant (MWI) or to the waste collection facility
LCA: Scenarios and additional technical information
Name Value Unit
Characteristic product properties of biogenic carbon
Litres of fuel (truck, EURO 0-6 mix) 0.0095 l/100km
Transport distance 700 km
Name ValueUnit
Capacity utilisation (including empty runs) 55 %
kg
Biogenic carbon content in product at factory gate 0.3
C
Installation in the building (A5)
Biogenic carbon content in accompanying kg
0.05 Name Value Unit
packaging at factory gate C
Material loss 0.121 kg
1 kg biogenic Carbon is equivalent to 44/12 kg of CO
2 Polyethylene packaging waste and installation waste are
considered to be incinerated in a municipal waste incineration
plant. Cardboard packaging waste is going to be recycled.
Preparation of the floor and auxiliaries (adhesives, fixing
agents, PET connectors etc.) are not taken into account.
Transport to the construction site (A4)
Maintenance (B2)
The values for cleaning refer to 1 m2 floor covering per year.
Depending on the application based on ISO 10874, the
3 Environmental Product Declaration - Interface - Superflor II, Needled tiles with a total pile weight of 521 g/m² and a CQuest Bio backing
technical service life recommended by the manufacturer and
End of Life (C1-C4)
the anticipated strain on the floor by customers, the case-
Three different end-of-life scenarios are declared and the
specific useful life can be established. Based on this useful life
results are indicated separately in module C.
the effects of module B2 need to be calculated in order to
Each scenario is calculated as a 100% scenario.
obtain the overall environmental impacts.
Scenario 1: 100 % landfill disposal
Name Value Unit Scenario 2: 100 % municipal waste incineration (MWI)
Maintenance cycle (vacuum cleaning) 208 Number /year with R1 > 0.6
Maintenance cycle (wet cleaning) 1,5 Number /year Scenario 3: 100 % recovery in the cement industry
Water consumption (wet cleaning) 0.004 m3
If combinations of these scenarios have to be calculated this
Cleaning agent (wet cleaning) 0.09 kg
should be done according to the following scheme:
Electricity consumption 0.314 kWh EOL-impact = x % impact (Scenario 1)
For further information on cleaning and maintenance see + y % impact (Scenario 2)
www.interface.com + z % impact (Scenario 3)
with x % + y % + z % = 100 %
Name ValueUnit
Service life Collected as mixed construction waste (scenario 1
4.045 kg
and 2)
Name Value Unit
Collected separately waste type (scenario 3) 4.045 kg
Life Span (according to
15 a
manufacturer's warranty) Landfilling (scenario 1) 4.045 kg
Corresponds to the Energy recovery (scenario 2) 4.045 kg
Declared product properties (at
specifications of EN - Energy recovery (scenario 3) 1.621 kg
the gate) and finishes
1307 Recycling (scenario 3) 2.424 kg
An assumed quality of work,
Conforms to the Reuse, recovery and/or recycling potentials (D), relevant
when installed in accordance
manufacturer's - scenario information
with the manufacturer’s
instructions Recovery or recycling potentials due to the three end-of-life
instructions
scenarios (module C) are indicated separately.
Usage conditions, e.g. Use in areas defined by
frequency of use, mechanical the use class according - Recycling in the cement industry (scenario 3) The organic
exposure to EN 1307 material of the carpet is used as an alternative fuel in a cement
Maintenance e.g. required According to the kiln. It mainly substitutes for lignite (68.8%), hard coal (23.6%)
frequency, type and quality and manufacturers - and petrol coke (7.6%). The inorganic material is substantially
replacement of components instructions integrated into the cement clinker and substitutes for original
material input. VDZ e.V.
4 Environmental Product Declaration - Interface - Superflor II, Needled tiles with a total pile weight of 521 g/m² and a CQuest Bio backing
LCA: Results
The LCA results refer to the declared product with a total pile weight of 521 g/m2. The declared result figures in module B2 have to be
multiplied by the assumed service life (in years) of the floor covering in the building under consideration.
Information on non-relevant modules: Modules B3 - B7 are not relevant during the service life of the carpet.
Modules C1, C3/1, C4/2 and C4/3 cause no additional impact (see chapter "LCA: Calculation rules" in this document). All these
modules are declared and marked as 'modules not relevant/declared'. Module C2 represents the transport for scenarios 1, 2 and 3.
Column D represents benefits from module A5 assembly.
DESCRIPTION OF THE SYSTEM BOUNDARY (X = INCLUDED IN LCA; ND = MODULE OR INDICATOR NOT DECLARED; MNR =
MODULE NOT RELEVANT)
Benefits and
Construction loads beyond
Product stage Use stage End of life stage
process stage the system
boundaries
la ire ta m w a Ry lp p u s tro p s n a rT g n iru tc a fu n a M e h t m o rf tro p s n a rTe tis e h t o t e ta g y lb m e s s A e s U e c n a n e tn ia M ria p e R tn e m e c a lp e R tn e m h s ib ru fe R y g re n e la n o ita re p Oe s u re ta w la n o ita re p Oe s u n o itc u rts n o c -e Dn o itilo m e d tro p s n a rT g n is s e c o rp e ts a W la s o p s iD -e s u e R-y re v o c e R-g n ilc y c e Rla itn e to p
A1 A2 A3 A4 A5 B1 B2 B3 B4 B5 B6 B7 C1 C2 C3 C4 D
X X X X X X X MNR MNR MNR MND MND X X X X X
RESULTS OF THE LCA - ENVIRONMENTAL IMPACT according to EN 15804+A2: 1 m² floor covering
Parameter Unit A1-A3 A4 A5 B1 B2 C1 C2 C3/2 C3/3 C4/1 D D/1 D/2 D/3
-1.04E
GWP-total kg CO 2 eq 6.11E+00 2.48E-01 3.76E-01 0 5.49E-01 0 1.37E-02 4.31E+004.36E+00 2.5E+00 -4.5E-02 0 +00 -2.52E-01
-1.04E
GWP-fossil kg CO 2 eq 7.38E+00 2.44E-01 3.54E-01 0 3.48E-01 0 1.35E-02 3.2E+00 3.25E+00 1.39E+00 -4.48E-02 0 +00 -2.52E-01
GWP- -1.28E
biogenic kg CO 2 eq +00 3.15E-03 2.19E-02 0 4.16E-03 0 1.74E-04 1.11E+00 1.11E+00 1.11E+00 -2.29E-04 0 -5.31E-03 -2.85E-04
GWP-luluc kg CO 2 eq 4.48E-03 1.38E-03 1.86E-04 0 1.96E-01 0 7.63E-05 2.46E-04 4.42E-04 1.4E-04 -4.92E-06 0 -1.14E-04 -1.05E-04
kg CFC11
ODP 1.37E-08 1.48E-14 4.1E-10 0 3.42E-08 0 8.2E-16 3.03E-13 6.08E-13 3.85E-13 -3.03E-13 0 -7.01E-12 -4.67E-13
eq
AP mol H+ eq 1.53E-02 1.47E-03 5.84E-04 0 8.32E-04 0 8.15E-05 2.52E-03 2.77E-03 8.5E-04 -5.89E-05 0 -1.36E-03 -7.3E-04
EP-
kg P eq 1.09E-04 7.38E-07 3.32E-06 0 5.19E-06 0 4.09E-08 8.41E-07 1E-06 5.35E-05 -6.16E-08 0 -1.43E-06 -2.49E-07
freshwater
EP-marine kg N eq 4.39E-03 7.23E-04 1.9E-04 0 1.97E-04 0 4E-05 1.16E-03 1.27E-03 1.88E-04 -1.6E-05 0 -3.7E-04 -2.48E-04
EP-terrestrial mol N eq 4.27E-02 8E-03 1.95E-03 0 2.83E-03 0 4.43E-04 1.31E-02 1.43E-02 2.06E-03 -1.71E-04 0 -3.97E-03 -2.71E-03
kg
POCP NMVOC 1.31E-02 1.37E-03 5.3E-04 4.18E-04 9.83E-04 0 7.57E-05 3E-03 3.21E-03 6.05E-04 -4.47E-05 0 -1.04E-03 -7.69E-04
eq
ADPE kg Sb eq 2.19E-06 2.07E-08 6.71E-08 0 2.3E-07 0 1.15E-09 2.29E-08 3.15E-08 1.99E-08 -6.75E-09 0 -1.57E-07 -2.25E-08
-1.77E -4.09E
ADPF MJ 1.6E+02 3.31E+004.98E+00 0 5.9E+00 0 1.83E-01 2.57E+00 3.4E+00 4.07E+00 -7.61E-01 0
+01 +01
m3 world
WDP eq 1.48E+01 2.21E-03 4.66E-01 0 9.99E-02 0 1.22E-04 6.05E-01 6.1E-01 -3.04E-03 -4.72E-03 0 -1.09E-01 -4.09E-02
deprived
GWP = Global warming potential; ODP = Depletion potential of the stratospheric ozone layer; AP = Acidification potential of land and water; EP =
Eutrophication potential; POCP = Formation potential of tropospheric ozone photochemical oxidants; ADPE = Abiotic depletion potential for non-fossil
resources; ADPF = Abiotic depletion potential for fossil resources; WDP = Water (user) deprivation potential)
RESULTS OF THE LCA - INDICATORS TO DESCRIBE RESOURCE USE according to EN 15804+A2: 1 m² floor covering
Parameter Unit A1-A3 A4 A5 B1 B2 C1 C2 C3/2 C3/3 C4/1 D D/1 D/2 D/3
PERE MJ 3.37E+01 1.88E-01 1.77E+00 0 3.69E+00 0 1.04E-02 1.62E+01 1.64E+01 3.34E-01 -2.09E-01 0 -4.84E+00 -2.8E-01
-1.57E -1.57E
PERM MJ 1.59E+01 0 -2.6E-01 0 0 0 0 0 0 0 0 0
+01 +01
PERT MJ 4.97E+01 1.88E-01 1.51E+00 0 3.69E+00 0 1.04E-02 4.66E-01 7.01E-01 3.34E-01 -2.09E-01 0 -4.84E+00 -2.8E-01
PENRE MJ 1.29E+02 3.31E+00 5.38E+00 0 5.9E+00 0 1.83E-01 3.32E+01 3.4E+01 4.07E+00 -7.61E-01 0 -1.77E+01-4.09E+01
-3.06E -3.06E
PENRM MJ 3.1E+01 0 -3.96E-01 0 0 0 0 0 0 0 0 0
+01 +01
PENRT MJ 1.6E+02 3.31E+00 4.99E+00 0 5.9E+00 0 1.83E-01 2.57E+00 3.4E+00 4.07E+00 -7.61E-01 0 -1.77E+01-4.09E+01
SM kg 2.57E+00 0 7.72E-02 0 0 0 0 0 0 0 0 0 0 2E-02
RSF MJ 0 0 0 0 0 0 0 0 0 0 0 0 0 0
NRSF MJ 0 0 0 0 0 0 0 0 0 0 0 0 0 0
FW m3 3.69E-01 2.12E-04 1.16E-02 0 3.34E-03 0 1.18E-05 1.43E-02 1.45E-02 4.76E-05 -2E-04 0 -4.63E-03 -3.55E-03
PERE = Use of renewable primary energy excluding renewable primary energy resources used as raw materials; PERM = Use of renewable primary
energy resources used as raw materials; PERT = Total use of renewable primary energy resources; PENRE = Use of non-renewable primary energy
excluding non-renewable primary energy resources used as raw materials; PENRM = Use of non-renewable primary energy resources used as raw
materials; PENRT = Total use of non-renewable primary energy resources; SM = Use of secondary material; RSF = Use of renewable secondary fuels;
NRSF = Use of non-renewable secondary fuels; FW = Use of net fresh water
5 Environmental Product Declaration - Interface - Superflor II, Needled tiles with a total pile weight of 521 g/m² and a CQuest Bio backing
RESULTS OF THE LCA – WASTE CATEGORIES AND OUTPUT FLOWS according to EN 15804+A2:
1 m² floor covering
Parameter Unit A1-A3 A4 A5 B1 B2 C1 C2 C3/2 C3/3 C4/1 D D/1 D/2 D/3
HWD kg 2.26E-07 1.59E-11 6.79E-09 0 4.19E-05 0 8.78E-13 3.67E-10 4.02E-10 6.27E-10 -1.03E-10 0 -2.39E-09 -7.02E-11
NHWD kg 1.19E-01 4.75E-04 4.02E-02 0 7.3E-03 0 2.63E-05 1.21E+00 1.21E+00 4.03E+00 -3.85E-04 0 -8.92E-03 -7.89E-04
RWD kg 4.13E-03 4.08E-06 1.27E-04 0 3.76E-04 0 2.26E-07 1.03E-04 1.64E-04 5E-05 -5.99E-05 0 -1.39E-03 -5.59E-05
CRU kg 0 0 0 0 0 0 0 0 0 0 0 0 0 0
MFR kg 0 0 1.21E-01 0 0 0 0 0 1.37E+00 0 0 0 0 0
MER kg 0 0 0 0 0 0 0 0 0 0 0 0 0 0
EEE MJ 0 0 1.87E-01 0 0 0 0 4.17E+00 0 0 0 0 0 0
EET MJ 0 0 3.49E-01 0 0 0 0 8E+00 4.84E+01 0 0 0 0 0
HWD = Hazardous waste disposed; NHWD = Non-hazardous waste disposed; RWD = Radioactive waste disposed; CRU = Components for re-use;
MFR = Materials for recycling; MER = Materials for energy recovery; EEE = Exported electrical energy; EET = Exported thermal energy
RESULTS OF THE LCA – additional impact categories according to EN 15804+A2-optional:
1 m² floor covering
Parameter Unit A1-A3 A4 A5 B1 B2 C1 C2 C3/2 C3/3 C4/1 D D/1 D/2 D/3
Disease
PM 1.22E-07 8.51E-09 4.49E-09 0 6.84E-08 0 4.71E-10 1.78E-08 1.94E-08 8.17E-09 -4.88E-10 0 0 -9.52E-09
incidence
kBq U235
IR 6.62E-01 5.98E-04 2.04E-02 0 6.78E-02 0 3.31E-05 1.57E-02 2.59E-02 7.38E-03 -1.02E-02 0 0 -4.81E-03
eq
ETP-fw CTUe 1.17E+02 2.29E+00 3.63E+00 3.6E-03 2.69E+00 0 1.27E-01 1.49E+00 1.97E+00 3.98E+00 -1.67E-01 0 0 -6.87E+00
HTP-c CTUh 2.54E-09 4.64E-11 7.99E-11 0 6.21E-10 0 2.57E-12 6.84E-11 7.95E-11 1.79E-10 -7.68E-12 0 0 -6.07E-11
HTP-nc CTUh 1.03E-07 2.75E-09 3.34E-09 2.6E-11 9.46E-09 0 1.52E-10 4.99E-09 5.55E-09 1.5E-08 -2.95E-10 0 0 -3.07E-09
SQP SQP ND ND ND ND ND ND ND ND ND ND ND ND ND ND
PM = Potential incidence of disease due to PM emissions; IR = Potential Human exposure efficiency relative to U235; ETP-fw = Potential comparative
Toxic Unit for ecosystems; HTP-c = Potential comparative Toxic Unit for humans (cancerogenic); HTP-nc = Potential comparative Toxic Unit for humans
(not cancerogenic); SQP = Potential soil quality index
No substantiated values can be given for the SQP indicator with the existing database.
The result figures given in module B2 refer to a period of 1 year because a reference service life is not declared. They have to be
multiplied by the assumed service life (in years) of the floor covering in the building under consideration.
Disclaimer 1 – for the indicator 'Potential Human exposure efficiency relative to U235'.
This impact category deals mainly with the eventual impact of low dose ionizingradiation on human health of the nuclear fuel cycle. It
does not consider effects due to possible nuclear accidents, occupational exposure nor due to radioactive waste disposal in
undergroundfacilities. Potential ionizing radiation from the soil, from radon and from some construction materials is also not measured
by this indicator.
Disclaimer 2 – for the indicators 'abiotic depletion potential for non-fossil resources', 'abiotic depletion potential for fossil resources',
'water (user) deprivation potential, deprivation-weighted water consumption', 'potential comparative toxic unit for ecosystems', 'potential
comparative toxic unit for humans – cancerogenic', 'Potential comparative toxic unit for humans - not cancerogenic', 'potential soil
quality index'.
The results of this environmental impact indicator shall be used with care as the uncertainties on these results are high or as there is
limited experienced with the indicator.
References
EN 1307 coverings – Environmental product declarations – Product
DIN EN 1307: 2014+A1:2016+A2:2018-05: Textile floor category rules
coverings - Classification
ISO 10874
EN 13501-1 DIN EN ISO 10874: 2012+A1:2021-04: Resilient, textile and
DIN EN 13501-1:2019-05: Fire classification of construction laminate floor coverings - Classification
products and building elements - Part 1: Classification using
data from reaction to fire tests ISO 14025
DIN EN /ISO 14025:2011-10/, Environmental labels and
EN 14041 declarations — Type III environmental declarations —
DIN EN 14041: 2018-05 and DIN EN 14041: 2008-05: Principles and procedures
Resilient, textile and laminate floor coverings - Essential
characteristics ISO 14040
DIN EN ISO 14040:2006+A1:2020 Environmental
EN 15804 management - Life cycle assessment - Principles and
DIN EN 15804:2012+A2:2019 + AC:2021, Sustainability of framework
construction works — Environmental Product Declarations —
Core rules for the product category of construction products ISO 14044
DIN EN ISO 14044:2006+A1:2018+A2:2020 Environmental
EN 16810 management - Life cycle assessment - Requirements and
DIN EN 16810: 2017-08: Resilient, textile and laminate floor guidelines
6 Environmental Product Declaration - Interface - Superflor II, Needled tiles with a total pile weight of 521 g/m² and a CQuest Bio backing
ISO 15686 GaBi database
ISO 15686: Buildings and constructed assets - Service life GaBi Software-System and Database for Life Cycle
planning ISO 15686-1: 2011-05: Part 1: General principles and Engineering, version 10.5 Sphera, Leinfelden-Echterdingen,
framework ISO 15686-2: 2012-05: Part 2: Service life prediction database version 2022-1
procedures ISO 15686-7: 2017-04: Part 7: Performance
evaluation for feedback of service life data from practice ISO PCR Part A
15686-8: 2008-06: Part 8: Reference service life and service- Product Category Rules for Building-Related Products and
life estimation Services Part A: Calculation Rules for the Life Cycle
Assessment and Requirements on the Project Report according
Regulation (EU) No. 305/2011 to EN 15804+A2:2019, V1.3, Berlin: Institut Bauen und Umwelt
Regulation No. 305/2011 Construction Products Regulation e.V. (IBU), August 2022
(CPR) of the European Council and of the European
Parliament, April 2011 PCR Part B
Product Category Rules for Building-Related Products and
General Instructions for the IBU-EPD Program Services Part B: Requirements on the EPD for floor coverings,
General Instructions for the EPD-Program of the Institut Bauen V1, Berlin: Institut Bauen und Umwelt e.V. (IBU), April 2023
und Umwelt e.V., The Preparation of Environmental Product
Declarations - EPDs, version 2.0, Institut Bauen und Umwelt PRODIS
e.V., Berlin, January 2021, www.ibu-epd.de Product Information System (PRODIS) of the European Carpet
Industry, Gemeinschaft umweltfreundlicher Teppichboden e.V
BNB, Nutzungsdauer von Bauteilen (GUT) and European Carpet and Rug Association
Bewertungssystem Nachhaltiges Bauen (BNB), Nutzungsdauer (ECRA), http://www.pro-dis.info
von Bauteilen, Bundesministerium des Inneren, für Bau und
Heimat, 24.02.2017 REACH
Regulation (EC) No 1907/2006 of the European Parliament and
ECHA candidate list of the Council of 18 December 2006 concerning the
Candidate List of substances of very high concern (SVHCs) for Registration, Evaluation, Authorisation and Restriction of
authorisation, 08.07.2021, European Chemicals Agency Chemicals (REACH), June 2017, last update: 17.01.2023
(ECHA), Helsinki, Finland
VDZ e.V.
ecoinvent Association of German Cement Works, Ed. Environ-mental
ecoinvent, Zurich, Switzerland, database version 3.7, published Data of the German Cement Industry 2020
September 2020
7 Environmental Product Declaration - Interface - Superflor II, Needled tiles with a total pile weight of 521 g/m² and a CQuest Bio backing
Publisher
Institut Bauen und Umwelt e.V. +49 (0)30 3087748- 0
Hegelplatz 1 info@ibu-epd.com
10117 Berlin www.ibu-epd.com
Germany
Programme holder
Institut Bauen und Umwelt e.V. +49 (0)30 3087748- 0
Hegelplatz 1 info@ibu-epd.com
10117 Berlin www.ibu-epd.com
Germany
Author of the Life Cycle Assessment
Gemeinschaft umweltfreundlicher Teppichboden +49 (0)241 96843 410
(GUT) e.V. mail@gut-ev.de
Schönebergstraße 2 www.gut-ev.org
52068 Aachen
Germany
Owner of the Declaration
Interface Europe Manufacturing BV +31 33 277 55 55
Industrielaan 15 receptie@interface.com
3925ZG Scherpenzeel www.interface.com
Netherlands
8 Environmental Product Declaration - Interface - Superflor II, Needled tiles with a total pile weight of 521 g/m² and a CQuest Bio backing
