ENVIRONMENTAL PRODUCT DECLARATION
as per ISO 14025 and EN 15804+A2
Owner of the Declaration Shaw Contract (Shaw Europe Ltd.)
Publisher Institut Bauen und Umwelt e.V. (IBU)
Programme holder Institut Bauen und Umwelt e.V. (IBU)
Declaration number EPD-SHA-20230448-CBA1-EN
Issue date 06.11.2023
Valid to 05.11.2028
TaskWorx® Carpet Tile with Polyamide 6 (Aquafil) Face Fibre
Shaw Contract (Shaw Europe Ltd.)
www.ibu-epd.com | https://epd-online.com
General Information
Shaw Contract (Shaw Europe Ltd.) TaskWorx® Carpet Tile with Polyamide 6 (Aquafil)
Face Fibre
Programme holder Owner of the declaration
IBU – Institut Bauen und Umwelt e.V. Shaw Contract (Shaw Europe Ltd.)
Hegelplatz 1 Blackaddie Road *
10117 Berlin DG46DB Sanquhar
Germany United Kingdom
Declaration number Declared product / declared unit
EPD-SHA-20230448-CBA1-EN 1 m2 of installed TaskWorx® Carpet Tile
This declaration is based on the product category rules: Scope:
Floor coverings, 01.08.2021 A Life Cycle Assessment (LCA) was conducted based upon production
(PCR checked and approved by the SVR) data collected from Shaw Contract (Shaw Europe, Ltd.), Plant SQ
manufacturing facility (Blackaddie Road, Sanquhar, DG46DB), located in
Scotland, UK. Production data was collected for TaskWorx® Carpet Tile
Issue date with Polyamide 6 (Aquafil) Face Fibre, for the period of one year, from
January to December 2021.
06.11.2023
This EPD is cradle-to-gate with options in scope with additional modules
A4, A5, B1 and B2. The EPD is created in accordance to the specifications
Valid to
of EN 15804+A2.
05.11.2028
The functional unit has been defined as 1m2 of installed TaskWorx® Carpet
Tile.
The EPD was generated with the help of Envision LCA Tool, version 1. The
tool has not been manipulated in calculating impact results. The current
version of the tool is maintained, saved, and stored for 10 years to be used
for revision and re-traceability purposes.
The owner of the declaration shall be liable for the underlying information
and evidence; the IBU shall not be liable with respect to manufacturer
information, life cycle assessment data and evidences.
Dipl.-Ing. Hans Peters The EPD was created according to the specifications of EN 15804+A2. In
(Chairman of Institut Bauen und Umwelt e.V.) the following, the standard will be simplified as EN 15804.
Verification
The standard EN 15804 serves as the core PCR
Independent verification of the declaration and data according to ISO
14025:2011
internally X externally
Florian Pronold Mrs Kim Allbury,
(Managing Director Institut Bauen und Umwelt e.V.) (Independent verifier)
1 Environmental Product Declaration - Shaw Contract (Shaw Europe Ltd.) - TaskWorx® Carpet Tile with Polyamide 6 (Aquafil) Face Fibre
Product
Other technical data parameters listed in IBU PCR Part B are
Product description/Product definition not relevant and, therefore, have not been declared.
This EPD applies to carpet tile with TaskWorx® backing system
together with Polyamide 6 (Aquafil) face fibre. Performance data of the product in accordance with the
declaration of performance with respect to its essential
TaskWorx® is a commercial carpet tile, for use as a floor characteristics according to 14041:2004A/C:2006.
covering in accordance with the manufacturer's guidelines.
Base materials/Ancillary materials
The carpet tile consists of Shaw’s unique facefibre, Polyamide TaskWorx® Carpet Tile with Polyamide 6 (Aquafil) Face Fibre is
6 (Aquafil), manufactured without recycled material on the comprised of the following raw materials:
TaskWorx® backing system, a modified bitumen compound with • 55-70% Calcium Carbonate, containing Recycled
100% natural recycled mineral filler, and a fibreglass Content
reinforcement layer. • 15-20% Modified Bitumen Polymer
• 10-15% Solution-dyed Polyamide 6 (Aqufil) Face Fibre
The Polyamide 6 (Aquafil) face fibre is tufted into a primary • 3-5% Styrene Butadiene Co-Polymer Latex
backing sheet containing recycled content. Latex is added to • 2-5% Polyester Primary & Secondary Backing
anchor the fibre andthe TaskWorx® backing system is then • 1-2% Fibreglass Reinforcement
applied. • 0-0.30% Anti-stat
The product is packaged in cardboard boxes, wrapped in
TaskWorx® is suitable for use in all commercial settings. It has plastic, and stacked on wooden pallets for distribution.
a life span of 15 years, and it comes with a 15-yearwarranty
(subject only to installation and maintenance being carried out The product fits into the defined scope and all raw material
inline with manufacturer’s guidelines). inputs, with no exceptions, are captured by the Envision LCA
Tool, version 1.
The product meets both internal and externalperformance
standards including those established in the EU under EN 1307 This product contains substances listed in the candidate list
andEN 10874 for a product suitable for heavy and general (date: 17.01.2023) exceeding 0.1 percentage by mass: no
commercial installations. For the placing on the market of the
product in the European Union/European Free Trade This product contains other CMR substances in categories 1A
Association (EU/EFTA) (with the exception ofSwitzerland), or 1B which are not on the candidate list, exceeding 0.1
Regulation (EU) No. 305/2011 (CPR) applies. The product percentage by mass: no
needs adeclaration of performance taking into consideration EN
14041:2004A/C:2006, andthe CE-marking. Biocide products were added to this construction product or it
has been treated with biocide products (this then concerns a
For the application and use, the respectivenational provisions treated product as defined by the (EU) Ordinance on Biocide
apply. Products No. 528/2012): no
Application Reference service life
TaskWorx® Carpet Tile with Polyamide 6 (Aquafil) Face Fibre is When properly installed as a commercial floor covering,
suitable for use as a floor covering in heavy and general TaskWorx® with Polyamide 6 (Aqufil) face fibre has a reference
commercial installations. service life of 15 years. This carpet tile product comes with a
15-year warranty, subject only to installation and maintenance
Technical Data being carried out in accordance with the manufacturer's
The technical specifications of the product are listed on the guidelines.
product's specification sheet, found at www.shawcontract.com.
This product meets the requirements of the harmonized
European Norm (hEN): EN14041:2004A/C:2006. Declarations
of performance related to fire, electrostatic, formaldehyde
emissions, and slip resistance can be found on the product's
specification sheet.
Constructional data
Name Value Unit
Product thickness 5.3 mm
Grammage 3900 g/m2
Product Form Carpet Tile -
Yarn type - Solution-dyed 0% Post-industrial
-
Polyamide 6 (Aquafil) Recycled Content
Total thickness 5.3 mm
Total carpet weight 3900 g/m2
Surface pile thickness 2.1 mm
Surface pile weight - Nominal
450 g/m2
Pile Mass
Length and width of squared
495 - 571 mm
elements
2 Environmental Product Declaration - Shaw Contract (Shaw Europe Ltd.) - TaskWorx® Carpet Tile with Polyamide 6 (Aquafil) Face Fibre
LCA: Calculation rules
• Module B3 - Repair (module not relevant).
Declared Unit • Module B4 - Replacement (module not relevant).
The declaration refers to the declared unit of 1 m² of installed • Module B5 - Refurbishment (module not relevant).
carpet tile. • Module B6 - Operational Energy Use (module not
Declared unit relevant).
• Module B7 - Operational Water Use (module not
Name Value Unit
relevant).
Declared unit 1 m2 End of Life Stage:
Grammage 3.901 kg/m2 Three scenarios have been evaluated:
Layer thickness 0.0053 m Scenario 1: the TaskWorx® carpet is 100% disposed of in a
landfill.
System boundary Scenario 2: the TaskWorx® carpet is 100% incinerated.
The type of EPD is Cradle-to-Gate with options modules C1– Scenario 3: 40% of TaskWorx® carpets are incinerated and the
C4, module D, and additional modules. The additional modules remaining 60% are landfilled. This assumption is based on the
are A4, A5, B1 and B2. carpet disposal rates in Europe mentioned in the study
conducted by Deutsche Umwelthilfe in 2017 (Umwelthilfe,
The modules considered in the life cycle assessment and 2017) and the European Commission in 2013 (Commission,
environmental product declaration, based on the product's 2013).
entire life cycle, are described as follows: • Module C1 - The carpet is de-constructed manually and
no additional environmental impact is caused.
Production Stage: • Module C2 - Transport of the carpet waste to a landfill or
• Module A1 - Provision of Raw Materials. to the municipal waste incineration plant.
• Module A2 - Transport of Raw Materials. • Module C3 - Impacts from thermal treatment disposal
• Module A3 - Manufacturing. (C3/2 and C3/3).
Construction/Installation Stage: • Module C4 - Impacts from landfill disposal (C4/1 and
C4/3).
• Module A4 - Transportation by truck of the product to the
Module D includes benefits from energy recovery via treatment
construction site in Europe.
of packaging materials and incineration of carpets at their end
• Module A5 - Installation of the carpet, treatment of
of life (D/1, D/2 and D/3), as well as the burdens of balancing
cutting waste (landfill) and packaging waste (landfill,
the secondary material content in modules A1 and A3 via the
recycling, and incineration). The production of the
net-scrap approach.
amount of carpet that occurs as installation waste is
also included along with its transport to the place of Geographic Representativeness
installation. Biogenic carbon that is stored in the wooden Land or region, in which the declared product system is
pallets and cardboard (packaging) is released as carbon manufactured, used or handled at the end of the product´s
dioxide emissions into the air at the end of life in module lifespan: Europe
A5.
Use Stage:
Comparability
• Module B1 - Indoor emissions of volatile organic
Basically, a comparison or an evaluation of EPD data is only
compounds (VOCs) during the first few months after
possible if all the data sets to be compared were created
installation.
according to EN 15804 and the building context, respectively
• Module B2 - Carpet cleaning per year, including
the product-specific characteristics of performance, are taken
vacuuming (electricity consumption) and hot water
into account. The background database used for the creation of
cleaning (electricity and water consumption, as well as
the EPD: GaBi ts software, CUP 2022.2.
waste water treatment).
LCA: Scenarios and additional technical information
Name Value Unit
Characteristic product properties of biogenic carbon
Transport distance (truck) 687 km
Biogenic carbon is only present in packaging (wooden pallets
Capacity utilisation (including empty runs) 55 %
and cardboards). Assumed water content in wooden pallet
(packaging): 18%.
Installation in the building (A5)
Information on describing the Biogenic Carbon Content at The installation of TaskWorx® is done manually and no energy
factory gate
is required. A Pressure-Sensitive adhesive is required for the
Name ValueUnit installation of TaskWorx® carpet tile and should be used in
Biogenic carbon content in accompanying kg accordance with the manufacturer's guidelines. Installation
0.14
packaging C losses have been accounted for in module A5. Product losses
are considered as 5%.
The following technical scenario information is required for the
The packaging material treatment and disposal are also
declared modules and optional for non-declared modules.
considered in module A5 (landfill, recycling, and incineration)
Transport to the construction site (A4) and the resulting benefits from energy generation are included
in module D. The quantity of wooden pallets used is 0.133 kg
per m². Wooden pallets are assumed to be re-used 20
3 Environmental Product Declaration - Shaw Contract (Shaw Europe Ltd.) - TaskWorx® Carpet Tile with Polyamide 6 (Aquafil) Face Fibre
timesbefore being disposed of. Hence, the quantity of pallet
Reference service life
disposed is 0.007 kg. The quantity of cardboard packaging is
Name ValueUnit
0.21 kg/m² and the quantity of plastic packaging is 0.0103
kg/m². Total amount of packaging disposed at installation is Reference service life (according to ISO 15686-1, -
15 a
0.227 kg. Packaging disposal rates (Source: Eurostat, 2, -7 and -8)
Recovery and recycling rates for packaging). Life Span according to the manufacturer 15 a
• Paper - 82.8% recycled; 9.4% landfilled; and 7.8%
End of Life (C1-C4)
incinerated
C1 - The product dismantling from the building is done
• Plastic - 40.3% recycled; 28.7% landfilled; and 31.0%
manually without energy burden.
incinerated
C2 - Transportation of the product to the end of life is assumed
• Wood pallets - 39.8% recycled; 34.5% landfilled; and
to be 161 km (100 miles).
25.7% incinerated
C3/2 - The TaskWorx® carpet is 100% combusted in an
Name ValueUnit
incineration plant with energy recovery (R>0.6).
Auxiliary 0.23 kg C3/3 - It is assumed that 40% of TaskWorx® carpets are
Material loss 0.195 kg incinerated and the remaining 60% are landfilled.
Output substances following waste treatment on C4/1 - The TaskWorx® carpet is 100% disposed of in landfill.
0.227 kg
site (packaging materials) C4/3 - It is assumed that 40% of TaskWorx® carpets are
incinerated and the remaining 60% are landfilled.
Use (B1) see cap. 2.12 use
Name ValueUnit
Name Value Unit Collected as mixed construction wastee 3.901 kg
Emissions to air (TVOC) after 50 days - Indoor Air 900 mg/m² Landfilling (Scenario 1 - C3/1, C4/1 and D/1) 3.901 kg
Comfort Gold®
Incineration (Scenario 2 - C3/2, C4/2, and D/2) 3.901 kg
Emission testing was conducted in accordance to Eurofins Landfilling (60%) and Incineration (40%) (Scenario
Indoor Air Comfort Gold® certification. After 28 days, the 3 - C3/3, C4/3 and D/3) 3.901 kg
specific concentration of TVOCs was <100 ug/m3, as required
by the certification standard.
Reuse, recovery and/or recycling potentials (D), relevant
scenario information
Maintenance (B2) For the thermal and electrical energy generated in Module A5
For the maintenance of TaskWorx® Carpet Tile, 2 hot water due to thermal treatment of packaging, avoided burdens have
extraction cleanings (water and electricity consumption) per been calculated by the inversion of electricity grid mix and
year as well as 52 vacuum cleanings (electricity consumption) thermal energy from natural gas, using European datasets.
per year are recommended. The Reference Service Life of the Module D also includes the environmental burdens linked to the
product is 15 years. The results in the EPD declare a supply to secondary materials (nylon and calcium carbonate)
maintenance for the period of 1 year. used in the carpet production.
Name Value Unit
Water consumption (1 year) 0.0009 m3
Electricity consumption (1 year) 0.772 kWh
4 Environmental Product Declaration - Shaw Contract (Shaw Europe Ltd.) - TaskWorx® Carpet Tile with Polyamide 6 (Aquafil) Face Fibre
LCA: Results
The B2 module declares the maintenance (cleaning) per one year. The user of the EPD will be able to scale the results for its entire
useful life by multiplying the impact by the RSL.
The LCA results presented below applies to 100% landfilled end of life scenario.
DESCRIPTION OF THE SYSTEM BOUNDARY (X = INCLUDED IN LCA; MND = MODULE OR INDICATOR NOT DECLARED; MNR
= MODULE NOT RELEVANT)
Benefits and
Construction loads beyond
Product stage Use stage End of life stage
process stage the system
boundaries
la ire ta m w a Ry lp p u s tro p s n a rT g n iru tc a fu n a M e h t m o rf tro p s n a rTe tis e h t o t e ta g y lb m e s s A e s U e c n a n e tn ia M ria p e R tn e m e c a lp e R tn e m h s ib ru fe R y g re n e la n o ita re p Oe s u re ta w la n o ita re p Oe s u n o itc u rts n o c -e Dn o itilo m e d tro p s n a rT g n is s e c o rp e ts a W la s o p s iD -e s u e R-y re v o c e R-g n ilc y c e Rla itn e to p
A1 A2 A3 A4 A5 B1 B2 B3 B4 B5 B6 B7 C1 C2 C3 C4 D
X X X X X X X MNR MNR MNR MND MND X X X X X
RESULTS OF THE LCA - ENVIRONMENTAL IMPACT according to EN 15804+A2: 1 m² TaskWorx® Carpet
Parameter Unit A1-A3 A4 A5 B1 B2 C1 C2 C3 C4 D
GWP-total kg CO 2 eq 5.73E+00 2.45E-01 4.08E-01 2.54E-04 2.89E-01 0 5.28E-02 0 2.74E-01 6.15E-04
GWP-fossil kg CO 2 eq 6.09E+00 2.44E-01 4.13E-01 2.54E-04 2.86E-01 0 5.26E-02 0 2.76E-01 -3.49E-03
GWP-
biogenic kg CO 2 eq -3.61E-01 -3.37E-04 -5.37E-03 0 3.05E-03 0 -7.27E-05 0 -2.94E-03 4.07E-03
GWP-luluc kg CO 2 eq 1.83E-03 1.36E-03 2.06E-04 0 6.06E-05 0 2.93E-04 0 1.35E-04 3.45E-05
ODP kg CFC11 eq 8.28E-09 1.46E-14 4.36E-10 0 4.19E-12 0 3.15E-15 0 3.71E-13 7.12E-14
AP mol H+ eq 1.28E-02 2.52E-04 1.09E-03 0 6.29E-04 0 5.42E-05 0 8.19E-04 1.7E-05
EP-
kg P eq 1.93E-05 7.29E-07 1.57E-05 0 1.4E-06 0 1.57E-07 0 5.16E-05 3.26E-08
freshwater
EP-marine kg N eq 3.07E-03 8.23E-05 2.36E-04 0 1.43E-04 0 1.77E-05 0 1.81E-04 1.48E-05
EP-terrestrial mol N eq 3.04E-02 9.8E-04 3.05E-03 0 1.48E-03 0 2.11E-04 0 1.99E-03 1.62E-04
kg NMVOC
POCP 1.03E-02 2.22E-04 8.77E-04 1.41E-05 3.82E-04 0 4.78E-05 0 5.83E-04 3.29E-05
eq
ADPE kg Sb eq 8.05E-07 2.04E-08 6.77E-08 0 7.8E-08 0 4.4E-09 0 1.92E-08 -1.73E-09
ADPF MJ 1.39E+02 3.26E+00 8.72E+00 0 5.19E+00 0 7.03E-01 0 3.92E+00 -1.92E-01
m3 world eq
WDP 3.58E-01 2.19E-03 8.86E-02 0 6.54E-02 0 4.72E-04 0 -2.73E-03 -4.38E-03
deprived
GWP = Global warming potential; ODP = Depletion potential of the stratospheric ozone layer; AP = Acidification potential of land and water; EP =
Eutrophication potential; POCP = Formation potential of tropospheric ozone photochemical oxidants; ADPE = Abiotic depletion potential for non-fossil
resources; ADPF = Abiotic depletion potential for fossil resources; WDP = Water (user) deprivation potential)
RESULTS OF THE LCA - INDICATORS TO DESCRIBE RESOURCE USE according to EN 15804+A2: 1 m² TaskWorx® Carpet
Parameter Unit A1-A3 A4 A5 B1 B2 C1 C2 C3 C4 D
PERE MJ 8.17E+00 1.95E-01 5.11E+00 0 2.88E+00 0 4E-02 0 3.23E-01 -1.22E-02
PERM MJ 5.31E+00 0 -4.19E+00 0 0 0 0 0 0 0
PERT MJ 1.35E+01 1.95E-01 9.21E-01 0 2.88E+00 0 4E-02 0 3.23E-01 -1.22E-02
PENRE MJ 9.86E+01 3.44E+00 1.57E+00 0 5.19E+00 0 7.05E-01 0 3.92E+00 -1.93E-01
PENRM MJ 4.83E+01 0 -3.17E-01 0 0 0 0 0 0 0
PENRT MJ 1.45E+02 3.44E+00 1.26E+00 0 5.19E+00 0 7.05E-01 0 3.92E+00 -1.93E-01
SM kg 2.35E+00 0 1.24E-01 0 0 0 0 0 0 -2.47E+00
RSF MJ 0 0 0 0 0 0 0 0 0 0
NRSF MJ 0 0 0 0 0 0 0 0 0 0
FW m3 2E-02 2.1E-04 9.13E-03 0 2.75E-03 0 4.52E-05 0 5.08E-05 -8.89E-05
PERE = Use of renewable primary energy excluding renewable primary energy resources used as raw materials; PERM = Use of renewable primary
energy resources used as raw materials; PERT = Total use of renewable primary energy resources; PENRE = Use of non-renewable primary energy
excluding non-renewable primary energy resources used as raw materials; PENRM = Use of non-renewable primary energy resources used as raw
materials; PENRT = Total use of non-renewable primary energy resources; SM = Use of secondary material; RSF = Use of renewable secondary fuels;
NRSF = Use of non-renewable secondary fuels; FW = Use of net fresh water
RESULTS OF THE LCA – WASTE CATEGORIES AND OUTPUT FLOWS according to EN 15804+A2:
1 m² TaskWorx® Carpet
Parameter Unit A1-A3 A4 A5 B1 B2 C1 C2 C3 C4 D
HWD kg 1.06E-05 1.57E-11 5.61E-07 0 4.49E-10 0 3.38E-12 0 6.05E-10 2.59E-11
NHWD kg 2.96E-01 4.69E-04 2.49E-01 0 4.77E-03 0 1.01E-04 0 3.89E+00 2.07E-05
RWD kg 2.92E-03 4.03E-06 1.74E-04 0 8.3E-04 0 8.68E-07 0 4.82E-05 -6.42E-06
CRU kg 0 0 0 0 0 0 0 0 0 0
5 Environmental Product Declaration - Shaw Contract (Shaw Europe Ltd.) - TaskWorx® Carpet Tile with Polyamide 6 (Aquafil) Face Fibre
MFR kg 0 0 1.81E-01 0 0 0 0 0 0 0
MER kg 0 0 0 0 0 0 0 0 0 0
EEE MJ 0 0 6.37E-02 0 0 0 0 0 0 0
EET MJ 0 0 9.77E-02 0 0 0 0 0 0 0
HWD = Hazardous waste disposed; NHWD = Non-hazardous waste disposed; RWD = Radioactive waste disposed; CRU = Components for re-use;
MFR = Materials for recycling; MER = Materials for energy recovery; EEE = Exported electrical energy; EET = Exported thermal energy
RESULTS OF THE LCA – additional impact categories according to EN 15804+A2-optional:
1 m² TaskWorx® Carpet
Parameter Unit A1-A3 A4 A5 B1 B2 C1 C2 C3 C4 D
Disease
PM 1.37E-07 1.45E-09 1.21E-08 0 5.21E-09 0 3.13E-10 0 7.87E-09 1.78E-08
incidence
IR kBq U235 eq 3.19E-01 5.9E-04 1.94E-02 0 1.41E-01 0 1.27E-04 0 7.12E-03 2.64E-03
ETP-fw CTUe 7.61E+01 2.27E+00 5.05E+00 1.15E-04 2.35E+00 0 4.88E-01 0 3.84E+00 -1.1E-01
HTP-c CTUh 2.17E-09 4.57E-11 1.51E-10 0 6.79E-11 0 9.84E-12 0 1.72E-10 -6.91E-13
HTP-nc CTUh 1.14E-07 2.37E-09 8.23E-09 3.07E-12 2.65E-09 0 5.11E-10 0 1.44E-08 1.26E-11
SQP SQP 1.05E+01 1.12E+00 1.1E+01 0 1.87E+00 0 2.42E-01 0 2.82E-01 -5.35E-01
PM = Potential incidence of disease due to PM emissions; IR = Potential Human exposure efficiency relative to U235; ETP-fw = Potential comparative
Toxic Unit for ecosystems; HTP-c = Potential comparative Toxic Unit for humans (cancerogenic); HTP-nc = Potential comparative Toxic Unit for humans
(not cancerogenic); SQP = Potential soil quality index
Disclaimer 1: For the indicator 'Potential Human exposure efficiency relative to U235". This impact category deals mainly with the
eventualimpact of low dose ionizing radiation on human health of the nuclear fuelcycle. It does not consider effects due to possible
nuclear accidents, occupationalexposure nor due to radioactive waste disposal in underground facilities.Potential ionizing radiation
from the soil, from radon and from someconstruction materials is also not measured by this indicator.
Disclaimer 2: For the indicators 'Abiotic depletionpotential for non-fossil resources', “Abiotic depletion potential for fossilresources”,
“Water (user) deprivation potential","Deprivation-weighted water consumption”, “Potential comparative toxicunit for ecosystems”,
“Potential comparative toxic unit for humans -cancerogenic”, “Potential comparative toxic unit for humans -non-carcinogenic”, “Potential
soil quality index”. The results of theseenvironmental impact indicators shall be used with care as the uncertainties onthese results are
high or as there is limited experienced with the indicators. This EPD was created using a software tool.
References
STANDARDS: life planning — Part 2: Service life prediction procedures.
EN 10874 ISO 15686
EN 10874:2009, Resilient, textile and laminate floor coverings ISO 15686-7:2011, Building and constructed assets — Service
— Classification. life planning — Part 7: Performance evaluation for feedback of
service life data from practice.
EN 1307
EN 1307:2014, Textile floor coverings — Classification. ISO 15686
ISO 15686-8:2011, Building and constructed assets — Service
EN 14041 life planning — Part 8: Reference service life and service life
EN 14041:2004/AC:2006 — Resilient, textile and laminate floor estimation.
coverings — Essential characteristics.
FURTHER REFERENCES:
EN 15804
EN 15804:2012+A2:2019/AC:2021, Sustainability of Candidate list
construction works — Environmental product declarations — Candidate List of substances of very high concern for
Core rules for the product category of construction products. Authorisation, published on ECHA website, latest version
17.01.2023 (https://echa.europa.eu/candidatelist-table).
ISO 14025
ISO 14025:2011, Environmental labels and declarations — Deutsche Umwelthilfe
Type III environmental declarations — Principles and Deutsche Umwelthilfe. Swept under the Carpet: The Big Waste
procedures. Problem of the Carpet Industry in Germany, 2017.
ISO 14040 Envision LCA Tool
ISO 14040:2006, Environmental management — Life cycle Envision LCA Tool, 2021, Sphera Solutions GmbH, Leinfelden-
assessment — Principles and framework. Echterdingen, with acknowledgement of LBP University of
Stuttgart, version 1.
ISO 14044
ISO 14044:2006, Environmental management — Life cycle GaBi
assessment — Requirements and guidelines. GaBi Software System and Database for Life Cycle
Engineering, 1992-2021, Sphera Solutions GmbH, Leinfelden-
ISO 15686 Echterdingen, with acknowledgement of LBP University of
ISO 15686-1:2011, Building and constructed assets — Service Stuttgart, program version GaBi 10; database version 2021.1.
life planning — Part 1: General principles and framework.
GaBi documentation
ISO 15686 GaBi dataset documentation for the software system and
ISO 15686-2:2011, Building and constructed assets — Service databases, LBP, University of Stuttgart and Sphera Solutions
6 Environmental Product Declaration - Shaw Contract (Shaw Europe Ltd.) - TaskWorx® Carpet Tile with Polyamide 6 (Aquafil) Face Fibre
GmbH, Leinfelden-Echterdingen, 2021 (http://www.gabi-
software.com/support/gabi/gabi-database-2021-lci- PCR Part B
documentation/). Product Category Rules for Building Products, Part B:
Requirements on the EPD for floor coverings, version 1.7, 2022
IBU 2021 (www.bau-umwelt.de).
Institut Bauen und Umwelt e.V.: General Instructions for the
EPD programme of Institut Bauen und Umwelt e.V., Version Packaging disposal rates
2.0, Berlin: Institut Bauen und Umwelt e.V., 2021 (www.ibu- Eurostat, Recovery and recycling rates for packaging. 2015
epd.com). (http://ec.europa.eu/eurostat/web/environment/waste/main-
tables).
PCR Part A The literature referred to in the Environmental Product
PCR Part A: Calculation rules for the Life Cycle Assessment Declaration must be listed in full.Standards already fully quoted
and Requirements on the Background Report according to EN in the EPD do not need to be listed here again.
15804:2012+A2:2019/AC:2021, Version 1.3, Institut Bauen und The current version of PCR Part A and PCR Part B of the PCR
Umwelt e.V., 2021. document on which they are based must be referenced.
7 Environmental Product Declaration - Shaw Contract (Shaw Europe Ltd.) - TaskWorx® Carpet Tile with Polyamide 6 (Aquafil) Face Fibre
Publisher
Institut Bauen und Umwelt e.V. +49 (0)30 3087748- 0
Hegelplatz 1 info@ibu-epd.com
10117 Berlin www.ibu-epd.com
Germany
Programme holder
Institut Bauen und Umwelt e.V. +49 (0)30 3087748- 0
Hegelplatz 1 info@ibu-epd.com
10117 Berlin www.ibu-epd.com
Germany
Author of the Life Cycle Assessment
Sphera Solutions GmbH +49 711 341817-0
Hauptstraße 111- 113 info@sphera.com
70771 Leinfelden-Echterdingen www.sphera.com
Germany
Owner of the Declaration
Shaw Contract (Shaw Europe Ltd.) +1 800 257 7429
Blackaddie Road * infouk@shawcontract.com
DG46DB Sanquhar www.shawcontract.com
United Kingdom
8 Environmental Product Declaration - Shaw Contract (Shaw Europe Ltd.) - TaskWorx® Carpet Tile with Polyamide 6 (Aquafil) Face Fibre
