Environmental Product
Declaration
as per ISO 14025 and EN 15804+A2
Owner of the declaration: Tensar International Limited
Publisher: Kiwa-Ecobility Experts
Programme operator: Kiwa-Ecobility Experts
Registration number: EPD-TENSAR-217-EN (Rev.1_20.05.2022)
Issue date: 06.04.2022
Valid to: 06.04.2027
Tensar® TriAx® geogrid – TX150L-GD
High performance geogrid used for subgrade stabilisation solutions
1. General information
Tensar International Limited Tensar® TriAx® TX150L-GD
Programme holder Owner of the declaration
Kiwa-Ecobility Experts Tensar International Limited
Voltastr. 5 Units 2-4 Cunningham Court
13355 Berlin Shadsworth Business Park
Germany Blackburn, United Kingdom
Registration number Declared product / declared unit
EPD-TENSAR-217-EN (Rev.1_20.05.2022) 1 m2 geogrid
This declaration is based on the Product Scope
Category Rules Tensar® TriAx® TX150L-GD geogrid is a prod-
PCR B - Geosynthetic products 2022-02-08 uct of the product series TriAx TX100G. It is
(draft) produced and distributed by Tensar Interna-
Issue date tional Limited, located in Blackburn (United
06.04.2022 Kingdom). The EPD refers to the specific prod-
uct.
Valid to EPD type: Cradle to grave with options, and
06.04.2027 with modules C1-C4 and module D.
Kiwa-Ecobility Experts shall not be liable with
respect to manufacturer information, life cy-
cle assessment data and evidence.
Verification
The European standard EN 15804+A2:2019
serves as the core PCR.
Independent verification of the declaration
and data according to ISO 14025:2011-10
☐internal ☒external
Frank Huppertz
(Head of Kiwa-Ecobility Experts)
Prof. Dr. Frank Heimbecher Anne Kees Jeeninga - Advieslab V.o.f.
(Chairman of the independent expert committee Kiwa- (Third party verifier)
Ecobility Experts)
Page | 2 Tensar International Limited – Tensar® TriAx® TX150L-GD
2. Product
2.1 Product description
The geogrid is comprised of multiple hexagons formed by equilateral triangular apertures. These ap-
ertures are defined by a structure of monolithic, multidirectional tensile elements of defined orienta-
tion, size and shape.
The hexagonal geogrid is manufactured from an extruded polypropylene sheet, which is then punched
and orientated in three equilateral directions so that the resulting ribs of the triangular apertures have
a high degree of molecular orientation which continues through the mass of integral node.
The geogrid is supplied bonded with a geotextile to form a laminated geocomposite.
2.2 Application
The intended use of the geogrid is to stabilize granular layers in order to minimize deformations during
trafficking, to improve the load bearing capacity and to increase the design life of the granular layer in
or under a construction in roads, railways and other trafficked areas, taking into account prevailing
national regulations on design methodologies. The combination of the geogrid and the aggregate cre-
ates a mechanically stabilized composite layer with significantly improved properties and performance
capabilities in response to dynamic and static loading compared with aggregate layers alone. For some
conditions of use the geogrid is combined with a geotextile to form a geocomposite which can provide
additional or enhances intended uses. The additional or enhanced intended uses will primarily be fil-
tration or separation, or a combination of the two. When installing, the manufacturer’s installation
procedures shall be observed, as well as the respective national practices.
2.3 Technical data
Name Value Tolerance Unit
Weight of product /TR 041 B.3/ 410 -35 g/m2
Radial Secant Stiffness at 2% strain /TR 041 B. 1/ 290 -100 kN/m
Radial Secant Stiffness at 0,5% strain /TR 041 B.1/ 365 -90 kN/m
Radial Secant Stiffness Ratio /TR 041 B.1/ 0,75 -0,15 -
Junction Efficiency /TR 041 B.2/ 100 -10 %
Static Puncture Resistance /EN ISO 12236/ 1,64 -0,14 kN
Dynamic perforation resistance (Cone drop test)
26 5 mm
/EN ISO 13433
Characteristic Opening Size /EN ISO 12956/ 110 ±40 µm
Velocity Index
Water Permeability/EN ISO 11058/ 0,135 -0,035
(VIH50) ms-1
Hexagon Pitch /TR 041 B.4/ 120 ±6 mm
Maximum time for exposure after installa-
Resistance to weathering /EN 12224/
tion of 1 month
Resistant for 50 years when used in soil tem-
Resistance to oxidation and to acid and alkali liquids perature of 15°C and 100 years when used
/EN ISO 13438/ and /EN 14030/ in soil temperature of 15°C for soils with pH
between 4 and 9
Specific dimension of the finished rolls (width x
3,8 x 50 m x m
length)
Page | 3 Tensar International Limited – Tensar® TriAx® TX150L-GD
2.4 Placing on the market/ Application rules
For quality assurance the geogrids TriAx TX100-G series are regulated in accordance with the European
Technical Assessment (ETA) 12/0529 or EN 13249, 13250, 13251, 13253, 13254, 13255, 13257, 13265
and marked with a CE mark (or UKCA mark for the UK market) by the manufacturer. In the EU/EFTA
(excluding Switzerland) the placing of geogrids on the market is covered by Regulation (EU) No.
305/2011 of 9 March 2011. For the product use the respective national provisions shall apply. The
product is packed and transported as roll and mainly marketed in Europe.
2.5 Base materials / Ancillary materials
TriAx geogrids are manufactured from a homopolymer or a copolymer of Polypropylene (PP). PP is a
thermoplastic polymer. It belongs to the group of polyolefins and is partially crystalline and nonpolar.
PP is prepared by polymerisation of propene. It is rugged and unusually resistant to many chemical
solvents, bases and acids.
Raw material Unit Value
Polypropylene granules/pellets (PP) % 57
Masterbatch granules/pellets % 3
Geotextile % 40
There is no biogenic carbon in the products.
The product is not included in the “Candidate list of substances of very high concern for authorisation”
(SVHC).
2.6 Manufacturing
The manufacturing is located at Tensar Manufacturing Limited, 2 Sett End Road West, Blackburn, Lan-
cashire, BB1 2PU, United Kingdom. After this the extruded sheet passes the punching process. Depend-
ing on the specific product the punches differ in size. The punched sheet is then stretched. The result
is the specific triangular structure of each geogrid. The products are rolled and then packaged. Finally,
the geogrid is supplied bonded with a geotextile to form a laminated geocomposite.
The manufacturing process is shown in the following figure:
Figure 1: Process flow chart of the production of Tensar® TriAx® TX100-G series
Page | 4 Tensar International Limited – Tensar® TriAx® TX150L-GD
2.7 Packaging
Geogrids are rolled and banded twice with PP banding tape.
2.8 Reference Service Life (RSL)
The RSL of the stabilisation geogrid depends on the service life of the roadway or platform it is included
in. This is dependent on both the exact roadway structure and the intensity of usage. The stabilisation
geogrids can be used in both temporary and permanent roadways and platforms. For temporary ap-
plications, service life would be measured using anticipated trafficking or imposed loading and would
typically last for time durations measured in days, weeks or months. For permanent roadways, the
stabilisation geogrids will be required to provide a service life of around 20 years. According to the
manufacturer the reference service lifetime of the TriAx TX100-G series is approximately 100 years.
2.9 Other Information
For further information on TriAx TX100-G series products please visit the official Tensar International
Limited webpage under the following link: www.tensar.co.uk
Page | 5 Tensar International Limited – Tensar® TriAx® TX150L-GD
3. LCA: Calculation rules
3.1 Declared unit
In accordance with the PCR B 1 m2 of the specific geogrid is chosen as the declared unit.
Product Unit Value
Declared Unit m2 geogrid 1
Unit weight g/m2 429
Conversion factor to 1 kg - 2.33
3.2 System boundary
The Environmental Product Declaration is a complete life cycle with a functional unit. It considers all
potential environmental impacts of the product from the cradle to the end of life.
The manufacturing phase includes the production or extraction of the source materials, the transport
to the respective production plant and the production of the geogrids. All inputs (raw materials, pre-
cursors, energy and auxiliary materials) as well as the by-products and waste are considered for all life
cycle phases. Finally, only production-related energy consumption (excluding administration and social
rooms) is considered.
It is assumed that no activities for maintenance, repair, transport and replacement, refurbishment or
other material and energy flows take place during the useful life of 20 years (RSL). Modules B1 to B3
are therefore assumed to be zero. Product replacement (B4) and renovation (B5) only apply when the
product is considered in a lifespan (of a building, work, etc.). Operational water and energy use are not
considered.
The year 2020 represents the time reference for raw materials and electricity consumption. Due to the
production location United Kingdom is considered as the geographical reference area. However, envi-
ronmental effects such as the greenhouse effect can occur with a strong spatial and temporal offset.
The following production steps are considered during the manufacturing phase:
• Extraction and processing of the raw materials (PP, Masterbatch, Geotextile)
• Transport to the production site
• Processing of the geogrids (extrusion, punching, stretching, lamination)
• Packaging (including packaging material)
• End-of-life (including transport)
Secondary fuels are not included in the production process and are therefore not considered. The
waste materials and quantities produced are included in the respective modules.
3.3 Estimates and assumptions
Almost all datasets chosen for the LCA refer to the EU as the geographic reference. Transport dis-
tances for all raw materials used (raw materials, operating materials, packaging) could be recorded. A
payload factor of 50% was used for all truck transports (suppliers, disposal transports and internal
transports), which corresponds to a full delivery and empty return trip. A data set for a non-specific
truck was used.
The distance to the construction site (A4) was calculated according to the NMD (Nationale Milieu Da-
tabase (Dutch National Environmental Database)) method. Accordingly, the distance between the
Page | 6 Tensar International Limited – Tensar® TriAx® TX150L-GD
production site in Blackburn and Utrecht was considered (900 km). As the mean of transportation truck
(unspecified) was chosen.
Tensar International Limited switched in 2020 to a 100 % renewable wind energy. According to a wind
electricity portal, windbranche.de, 50% of wind power in UK is generated from onshore and 50% from
offshore wind parks. Based on this assumption an electricity data set was generated for the LCA calcu-
lation. No CO certificates were considered.
2
3.4 Cut-off criteria
All flows which influence the total mass, energy or environmental impact more than 1% are included
in the LCA. It can be assumed that the neglected processes would have contributed less than 5% to the
impact categories considered.
All process specific data could be determined and modelled by the use of generic data (EcoInvent 3.6)
The PP is bulk delivered in 24 tons batches – the pellets is blown into the silo. Therefore, there is no
packaging waste for the PP.
The masterbatch is delivered in octabins made of cardboard and a thin polythene liner. Cardboard and
liner are recycled afterwards. As the amounts for the masterbatch packaging are quite small referred
to the overall mass flow this packaging was neglected. It is assumed that the residues of the extrusion,
punching and stretching processes are less than 1% of the total mass, energy or environmental impact.
Therefore, these residues are within the cut-off criteria and were neglected.
3.5 Period under review
The production data applies to the operating year 2020.
3.6 Data quality
For all processes primary data was collected and provided by Tensar International Limited. The prima-
ry data refers to year 2020. For the data, which is not influenced by the manufacturer, generic data
was used. The secondary data was taken from the database EcoInvent (version 3.6). The database is
maintained on a regular basis and thus meets the requirements of EN 15804 (background data not
older than 10 years). The power sources were chosen from data for the UK in 2020, in accordance with
the geographical and time representativeness. The data quality is very good, because all process spe-
cific data could be documented and modelled by using the generic data.
RETHiNK EPD web application from the company NIBE was used to model the life cycle for the pro-
duction and disposal of the declared product systems. To ensure that the results are comparable, con-
sistent background data from the international database EcoInvent was used in the LCA (e.g. data rec-
ords on energy, transport, auxiliary materials and supplies). Almost all consistent data sets contained
in the EcoInvent database are documented and can be viewed online.
3.7 Allocation
Allocations were avoided as far as possible. Tensar uses PP for several products as a raw material and
all PP residues, which occur during the manufacturing, are recycled. The residues are not mandatorily
used again for the product from which they originate. The recycled residues might be used for products
from another PP based series.
For example: 5% residues of PP occur during the manufacturing of geogrid A. These 5% are recycled,
but due to operating conditions, it is possible that 4% is reused for geogrid A and 1% for geogrid B.
Page | 7 Tensar International Limited – Tensar® TriAx® TX150L-GD
For this calculation it was assumed, that the generated punchout and the regrind material of a specific
geogrid is reused in a closed loop recycling for the analysed geogrid. This was done to avoid product
specific shifts of potential environmental impacts. It was also assumed that the recycled PP substitutes
virgin PP after a regranulation and that this does not imply any quality losses.
3.8 Comparability
In principle, a comparison or assessment of the environmental impacts of different products is only
possible if they have been prepared in accordance with EN 15804. For the evaluation of the
comparability, the following aspects have to be considered in particular: PCR used, functional or
declared unit, geographical reference, definition of the system boundary, declared modules, data
selection (primary or secondary data, background database, data quality), scenarios used for use and
disposal phases, and the life cycle inventory (data collection, calculation methods, allocations, validity
period). For further guidance see EN 15804+A2 (5.3 Comparability of EPD for construction products).
Page | 8 Tensar International Limited – Tensar® TriAx® TX150L-GD
4. LCA: Scenarios and additional technical information
When installing stabilising geogrid, it is simply unrolled by hand on prepared subgrade or capping layer.
Apart from rolling out, no further installation measures are necessary, which would otherwise be re-
quired during road construction. A reject or unused portion of 5% of the stabilisation geogrid is as-
sumed during the installation process.
For C1 the process and amount of the generic dataset ‘Polyester weefsel’ (EN: polyester fabric) out of
chapter 22.46 Grondwapening en grondscheiding (EN: 22.46 Soil reinforcement and soil separation) of
the program DuboCalc with database version NMD version 1.8 - 5.01.14052018. In this generic dataset
0.0013 hrs of the process Gr.mach.hydr. (gemiddeld) (EN: Hydraulic excavator (average)) are stated for
module C1 (demolition).
For the end-of-life the NMD szenario PE/PP soil reinforcement (geotextile and geogrid) was chosen.
This scenario assumes that 25% of the geogrid remains in the subground, 70% are incinerated and 5%
are recycled. In the scenario the original waste scenario for benefits from recycling "Polyethylene,
HDPE, granulate | production (EU)" are substituted by the "Polypropene, granulate".
Note: The transport distances of the waste are based on the standard waste scenarios of the NMD
Determination Method (SBK 2019): incineration 150 km/ recycling 50 km / landfill 100 km; vehicle:
truck, unspecific. For energy recovery, it is assumed that only fossil raw materials are substituted, con-
sidering the calorific values of the raw materials of the declared product and energy and thermal effi-
ciencies of 18% and 32%. According the EN 15804, loads are credited in A3 or C3 to C4 and benefits
are credited in module D.
For all transports, the environmental profile of a non-specific truck transport was used (conservative
assumption): The vehicle operates with diesel, and it provides a fleet average that includes different
lorry classes as well as EURO classes. This environmental profile contains data for transport, which is
calculated for an average load factor, including empty return trips (EcoInvent 3.6).
5. LCA: Results
The following tables show the results of the impact assessment indicators, resource use, waste and
other output streams. The results presented here refer to the declared specific product.
Disclaimer on ADP-e, ADP-f, WDP, ETP-fw, HTP-c, HTP-nc, SQP: The results of these environmental
impact indicators must be used with caution, as the uncertainties in these results are high or as there
is limited experience with the indicator.
Disclaimer on IR: This impact category mainly addresses the potential effect of low dose ionizing radi-
ation on human health in the nuclear fuel cycle. It does not consider effects due to possible nuclear
accidents and occupational exposures, nor does it consider radioactive waste disposal in underground
facilities. Potential ionizing radiation from soil, radon, and some building materials is also not measured
by this indicator.
Page | 9 Tensar International Limited – Tensar® TriAx® TX150L-GD
Description of the system boundary
Construction process Benefits and loads beyond
Product stage Use stage End of life stage
stage the system boundaries
la ir e wta am Ry lp p u s t r o p s n a r T u n a M-g n ir u t c a f t r o p s n a r Tu n a m m o r-
f
o t r e r u t c a fe s u fo e c a lp n o it c u r t s n o
C
n o it a lla t s n -is s e c o r p e s U n ia M-e c n a n e t r ia p e R t n e m e c a lp e
R
r u fe R-n e m h s ib la n o it a r e p Oe s u y g r e n e la n o it a r e p Oe s u r e t a w e D- n o it c u r t s n o cn o it ilo m e d
/
t r o p s n a r T e t s a Wg n is s e c o r p la s o p s iD e s u e R-y r e v o c e R- g n ilc y c e R- a it n e t o pl
A1 A2 A3 A4 A5 B1 B2 B3 B4 B5 B6 B7 C1 C2 C3 C4 D
X X X X X X X X MND MND MND MND X X X X X
X=Module declared | MND=Module not declared
Results of the LCA – Environmental impact: 1 m2 Tensar® TriAx® TX150L-GD (EN 15804+A2)
Parameter Unit A1 A2 A3 A4 A5 B1 B2 B3 C1 C2 C3 C4 D
Core environmental impact indicators (EN 15804+A2/NMD set2)
ADP-mm kg Sb-eqv 5,23E-06 2,10E-07 4,06E-07 1,35E-06 4,35E-07 0,00E+00 0,00E+00 0,00E+00 1,04E-07 1,58E-07 1,03E-06 1,22E-08 -5,15E-07
ADP-f MJ 3,30E+01 1,50E-01 1,80E+00 8,02E-01 1,84E+00 0,00E+00 0,00E+00 0,00E+00 9,37E-01 9,39E-02 6,28E-01 2,69E-02 -9,45E+00
AP mol H+ eqv. 3,57E-03 1,40E-04 2,26E-04 3,08E-04 2,39E-04 0,00E+00 0,00E+00 0,00E+00 7,12E-04 3,61E-05 3,63E-04 9,92E-06 -5,47E-04
EP-fw kg PO4 eqv. 2,37E-05 8,74E-08 3,00E-06 5,36E-07 1,52E-06 0,00E+00 0,00E+00 0,00E+00 2,48E-07 6,28E-08 2,43E-06 2,04E-08 -1,17E-06
EP-m kg N eqv. 5,97E-04 3,67E-05 4,97E-05 1,09E-04 4,77E-05 0,00E+00 0,00E+00 0,00E+00 3,14E-04 1,27E-05 9,93E-05 6,01E-06 -1,43E-04
EP-t mol N eqv. 6,70E-03 4,07E-04 5,22E-04 1,20E-03 5,29E-04 0,00E+00 0,00E+00 0,00E+00 3,45E-03 1,40E-04 1,11E-03 3,65E-05 -1,59E-03
GWP-b kg CO2 eqv. 4,66E-05 1,59E-06 -5,31E-03 2,45E-05 6,58E-03 0,00E+00 0,00E+00 0,00E+00 1,89E-05 2,87E-06 1,17E-04 1,23E-05 -1,77E-04
GWP-f kg CO2 eqv. 1,01E+00 1,05E-02 1,05E-01 5,32E-02 1,09E-01 0,00E+00 0,00E+00 0,00E+00 6,81E-02 6,22E-03 8,06E-01 1,59E-02 -5,13E-01
GWP-luluc kg CO2 eqv. 2,63E-04 5,50E-06 1,31E-04 1,95E-05 2,51E-05 0,00E+00 0,00E+00 0,00E+00 5,37E-06 2,28E-06 6,55E-05 5,62E-07 -2,75E-05
GWP-total kg CO2 eqv. 1,01E+00 1,05E-02 9,94E-02 5,32E-02 1,15E-01 0,00E+00 0,00E+00 0,00E+00 6,81E-02 6,23E-03 8,06E-01 1,59E-02 -5,13E-01
ODP kg CFC 11 eqv. 2,15E-08 2,24E-09 1,10E-08 1,17E-08 3,97E-09 0,00E+00 0,00E+00 0,00E+00 1,47E-08 1,37E-09 2,46E-08 3,52E-10 -6,16E-08
kg NMVOC
POCP 3,18E-03 1,11E-04 1,78E-04 3,42E-04 2,14E-04 0,00E+00 0,00E+00 0,00E+00 9,49E-04 4,00E-05 2,97E-04 1,40E-05 -5,62E-04
eqv.
WDP m3 world eqv. 5,66E-01 4,59E-04 4,86E-02 2,87E-03 3,35E-02 0,00E+00 0,00E+00 0,00E+00 1,26E-03 3,36E-04 4,11E-02 1,15E-03 -6,58E-02
Additional environmental impact indicators (EN 15804+A2/NMD set 2)
ETP-fw CTUe 3,88E+00 1,24E-01 6,91E-01 7,15E-01 8,92E-01 0,00E+00 0,00E+00 0,00E+00 5,65E-01 8,37E-02 1,01E+01 2,86E-02 -7,51E-01
HTP-c CTUh 1,78E-10 5,32E-12 4,61E-11 2,32E-11 2,36E-11 0,00E+00 0,00E+00 0,00E+00 1,97E-11 2,71E-12 1,54E-10 7,51E-13 -3,93E-11
HTP-nc CTUh 5,70E-09 1,28E-10 6,91E-10 7,82E-10 5,71E-10 0,00E+00 0,00E+00 0,00E+00 4,85E-10 9,16E-11 3,20E-09 1,86E-11 -7,19E-10
IRP kBq U235 eqv. 1,54E-02 6,32E-04 1,58E-03 3,36E-03 1,24E-03 0,00E+00 0,00E+00 0,00E+00 4,02E-03 3,93E-04 2,57E-03 1,05E-04 -3,33E-03
disease in-
3,26E-08 7,40E-10 1,74E-09 4,78E-09 2,23E-09 0,00E+00 0,00E+00 0,00E+00 1,89E-08 5,60E-10 2,94E-09 1,87E-10 -2,56E-09
PM cidence
SQP 1,06E+00 9,84E-02 4,59E-01 6,95E-01 1,40E-01 0,00E+00 0,00E+00 0,00E+00 1,20E-01 8,14E-02 2,31E-01 6,36E-02 -5,08E-01
ADP-f=Depletion of abiotic resources-fossil fuels | ADP-mm=Depletion of abiotic resources- minerals and metals| AP=Acidification of soil and water | EP-fw =Eutrophication, freshwater | EP-m=Eutrophication marine | EP-T=Eutrophica-
tion, terrestrial | GWP-b=Global warming potential - Biogenic | GWP-f=Global warming potential - Fossil | GWP-luluc=Global warming potential - Land use and land use change |GWP-total=Global warming potential |ODP=Ozone layer
depletion |POCP=Photochemical oxidants creation | WDP=Water use | ETP-fw=Ecotoxicity, freshwater | HTP-c=Human toxicity, cancer | HTP-nc=Human toxicity, non-cancer | IRP=Ionising radiation, human health | PM=Particulate Matter
| SQP=Land use
Page | 10 Tensar International Limited – Tensar® TriAx® TX150L-GD
Results of the LCA – Resource use and environmental information: 1 m2 Tensar® TriAx® TX150L-GD (EN 15804+A2)
Parameter Unit A1 A2 A3 A4 A5 B1 B2 B3 C1 C2 C3 C4 D
PERE MJ 2,54E-01 1,67E-03 1,72E+00 1,00E-02 1,03E-01 0,00E+00 0,00E+00 0,00E+00 5,07E-03 1,18E-03 6,35E-02 4,76E-04 -1,08E-01
PERM MJ 0,00E+00 0,00E+00 7,27E-02 0,00E+00 3,64E-03 0,00E+00 0,00E+00 0,00E+00 0,00E+00 0,00E+00 0,00E+00 0,00E+00 -3,82E-03
PERT MJ 5,00E-01 1,67E-03 1,79E+00 1,00E-02 1,19E-01 0,00E+00 0,00E+00 0,00E+00 5,07E-03 1,18E-03 6,35E-02 4,76E-04 -1,12E-01
PENRE MJ 1,05E+01 1,59E-01 1,59E+00 8,51E-01 7,08E-01 0,00E+00 0,00E+00 0,00E+00 9,95E-01 9,97E-02 6,67E-01 2,86E-02 -9,57E+00
PENRM MJ 9,52E+00 0,00E+00 2,16E-01 0,00E+00 4,87E-01 0,00E+00 0,00E+00 0,00E+00 0,00E+00 0,00E+00 0,00E+00 0,00E+00 -8,52E-01
PENRT MJ 3,53E+01 1,59E-01 1,96E+00 8,51E-01 1,97E+00 0,00E+00 0,00E+00 0,00E+00 9,95E-01 9,97E-02 6,67E-01 2,86E-02 -1,04E+01
SM Kg 0,00E+00 0,00E+00 0,00E+00 0,00E+00 0,00E+00 0,00E+00 0,00E+00 0,00E+00 0,00E+00 0,00E+00 0,00E+00 0,00E+00 0,00E+00
RSF MJ 0,00E+00 0,00E+00 0,00E+00 0,00E+00 0,00E+00 0,00E+00 0,00E+00 0,00E+00 0,00E+00 0,00E+00 0,00E+00 0,00E+00 0,00E+00
NRSF MJ 0,00E+00 0,00E+00 0,00E+00 0,00E+00 0,00E+00 0,00E+00 0,00E+00 0,00E+00 0,00E+00 0,00E+00 0,00E+00 0,00E+00 0,00E+00
FW M3 1,04E-02 1,56E-05 1,22E-03 9,77E-05 6,65E-04 0,00E+00 0,00E+00 0,00E+00 4,83E-05 1,14E-05 1,21E-03 2,81E-05 -9,21E-04
HWD Kg 3,31E-06 3,12E-07 2,12E-06 2,03E-06 4,87E-07 0,00E+00 0,00E+00 0,00E+00 2,55E-06 2,38E-07 1,20E-06 4,09E-08 -1,00E-05
NHWD Kg 3,19E-02 6,88E-03 9,30E-03 5,09E-02 1,27E-02 0,00E+00 0,00E+00 0,00E+00 1,11E-03 5,95E-03 1,55E-02 1,08E-01 -4,61E-03
RWD Kg 1,49E-05 9,99E-07 1,73E-06 5,26E-06 1,34E-06 0,00E+00 0,00E+00 0,00E+00 6,51E-06 6,16E-07 2,26E-06 1,60E-07 -4,45E-06
CRU Kg 0,00E+00 0,00E+00 0,00E+00 0,00E+00 0,00E+00 0,00E+00 0,00E+00 0,00E+00 0,00E+00 0,00E+00 0,00E+00 0,00E+00 0,00E+00
MFR Kg 0,00E+00 0,00E+00 2,15E-04 0,00E+00 1,54E-03 0,00E+00 0,00E+00 0,00E+00 0,00E+00 0,00E+00 2,15E-02 0,00E+00 0,00E+00
MER Kg 0,00E+00 0,00E+00 0,00E+00 0,00E+00 0,00E+00 0,00E+00 0,00E+00 0,00E+00 0,00E+00 0,00E+00 0,00E+00 0,00E+00 0,00E+00
EE MJ 0,00E+00 0,00E+00 5,18E-02 0,00E+00 0,00E+00 0,00E+00 0,00E+00 0,00E+00 0,00E+00 0,00E+00 0,00E+00 0,00E+00 5,53E+00
PERE=renewable primary energy ex. raw materials | PERM=renewable primary energy used as raw materials | PERT=renewable primary energy total | PENRE=non-renewable primary energy ex. raw materials | PENRM=non-renewable
primary energy used as raw materials | PENRT=non-renewable primary energy total | SM=use of secondary material | RSF=use of renewable secondary fuels | NRSF=use of non-renewable secondary fuels | FW=use of net fresh water |
HWD=hazardous waste disposed | NHWD=non-hazardous waste disposed | RWD=radioactive waste disposed | CRU=Components for re-use | MFR=Materials for recycling | MER=Materials for energy recovery | EE=Exported energy
Results of the LCA – Environmental impact,optional: 1 m2 Tensar® TriAx® TX150L-GD (set 1 of the NMD determination method (version 1.0; July 2020))
Parameter Unit A1 A2 A3 A4 A5 B1 B2 B3 C1 C2 C3 C4 D
ADP-e Kg Sb 5,23E-06 2,10E-07 4,11E-07 1,35E-06 4,36E-07 0,00E+00 0,00E+00 0,00E+00 1,04E-07 1,58E-07 1,03E-06 1,22E-08 -5,15E-07
ADP-f Kg Sb 1,55E-02 7,22E-05 9,29E-04 3,88E-04 8,72E-04 0,00E+00 0,00E+00 0,00E+00 4,45E-04 4,54E-05 3,34E-04 1,31E-05 -5,00E-03
GWP Kg CO2 eqv. 9,68E-01 1,04E-02 1,03E-01 5,27E-02 1,07E-01 0,00E+00 0,00E+00 0,00E+00 6,74E-02 6,17E-03 8,04E-01 1,36E-02 -5,05E-01
ODP Kg CFC-11 eqv. 2,08E-08 1,78E-09 9,83E-09 9,35E-09 3,71E-09 0,00E+00 0,00E+00 0,00E+00 1,17E-08 1,09E-09 2,47E-08 2,81E-10 -5,44E-08
POCP Kg Ethene eqv. 8,65E-04 8,63E-06 3,71E-05 3,18E-05 4,96E-05 0,00E+00 0,00E+00 0,00E+00 6,86E-05 3,72E-06 2,87E-05 3,08E-06 -1,02E-04
AP Kg SO2 eqv. 2,98E-03 1,11E-04 1,83E-04 2,32E-04 1,96E-04 0,00E+00 0,00E+00 0,00E+00 5,08E-04 2,71E-05 2,83E-04 7,54E-06 -4,33E-04
EP Kg PO43- eqv. 2,94E-04 1,41E-05 3,04E-05 4,55E-05 2,28E-05 0,00E+00 0,00E+00 0,00E+00 1,15E-04 5,33E-06 4,61E-05 3,04E-06 -5,62E-05
HTP kg 1.4 DB 1,35E-01 4,91E-03 2,92E-02 2,22E-02 1,35E-02 0,00E+00 0,00E+00 0,00E+00 2,50E-02 2,60E-03 5,86E-02 1,11E-03 -3,04E-02
FAETP kg 1.4 DB 3,12E-03 1,18E-04 1,15E-03 6,48E-04 5,02E-04 0,00E+00 0,00E+00 0,00E+00 3,47E-04 7,59E-05 3,01E-03 1,16E-03 -3,75E-04
MAETP kg 1.4 DB 7,96E+00 4,58E-01 9,48E-01 2,33E+00 1,20E+00 0,00E+00 0,00E+00 0,00E+00 1,21E+00 2,73E-01 8,77E+00 1,16E+00 -1,47E+00
TETP kg 1.4 DB 5,51E-04 1,64E-05 2,69E-04 7,84E-05 5,58E-05 0,00E+00 0,00E+00 0,00E+00 4,11E-05 9,18E-06 1,50E-04 1,92E-06 -1,02E-04
ADP-e=Depletion of abiotic resources - elements | ADP-f=Depletion of abiotic resources - fossil fuels | GWP=Global warming potential | ODP=Ozone layer depletion | POCP=Photochemical oxidants creation | AP=Acidification of soil and
water | EP=Eutrophication | HTP=Human toxicity | FAETP=Ecotoxicity fresh water | MAETP=Ecotoxicity marine water | TETP=Ecotoxicity terrestric
Page | 11 Tensar International Limited – Tensar® TriAx® TX150L-GD
6. LCA: Interpretation
As shown in the figure below, raw material supply (A1) dominates in most environmental core
indicators, often followed by the production process (A3). In some environmental core indicators
demolition phase (C1) has a great impact. However, C1 is strongly dependent on the assumption (here
diesel consumption of a construction site vehicle). The highest influence on the Global Warming
Potential have row material supply (A1), waste processing (C3), and production process (A3).
Transports (A2, A4, C2) have rather a minor impact within all core indicators.
100%
80%
60%
40%
20%
0%
-20%
-40%
ADP-mm ADP-f AP EP-fw EP-m EP-T GWP-total ODP POCP WDP
A1 A2 A3 A4 A5 C1 C2 C3 C4 D
Figure 2: Tensar® TriAx® TX150L-GD - Impact of the individual modules on the environmental core
indicator
The MKI (Dutch: Milieukostenindicator) value calculated based on set 1 of the NMD determination
method amounts to 0.133.
The data quality can be classified as good overall. All relevant process-specific data could be collected
in the operational data collection. Consistent data sets from the EcoInvent database were available for
almost all inputs and outputs. The background data meet the requirements of EN 15804, and the pro-
duction data were recorded for the 2020 operating year. The quantities of raw materials and supplies
used as well as energy consumption were recorded for the entire operating year.
Page | 12 Tensar International Limited – Tensar® TriAx® TX150L-GD
7. Requisite evidence
In 2008 Tensar® TriAx® TX160 was tested concerning its leaching behaviour using the trough method.
Due to this method the institute “PrüftechnikCDL” could determine the direct environmental impacts
to the local environment (soil and groundwater). No parameters from the BundesBodenschutz-und
Altlastenverordnung (BBodSchV) were found in the 5. eluate, except from phenol. The analysed phenol
concentrations are with 12 µg below the threshold value of the BBodSchV. In accordance with the
criteria of the BBodSchV the environmental soundness of the geogrid could be confirmed. This result
can be transferred to all the other types of geogrids referring to the product series TX100G, so as well
to TriAx® TX150L-GD.
Page | 13 Tensar International Limited – Tensar® TriAx® TX150L-GD
8. References
CML-IA April 2013 – Charakterisierungsfaktoren entwickelt durch Institut of Environmental Sciences
(CML): Universität Leiden, Niederlande - http://www.cml.leiden.edu/software/data-cmlia.html
Donndorf, R., Kahle H., Müller, G., Philipp H-J., Taschow, H-J., Wolf, O. (1973): Werkstoffeinsatz und
Korrosionsschutz in der chemischen Industrie. VEB Deutscher Verlag für Grundstoffindustrie Leip-zig.
European Commission Joint Research Centre Institute for Prospective Technological Studies (JCR
2014): End-of-waste criteria for waste plastic for conversion, Seville, 2014, doi:10.2791/13033
Klöpffer, W., Grahl B.: Ökobilanz (LCA) – Ein Leitfaden für die Ausbildung und Beruf, Wily-VCH Ver-
lag, Weinheim, 2007
Rosauer, V. (2010): Abschätzung der herstellungsbedingten Qualität und Lebensdauer von Asphalt-
deckschichten mit Hilfe der Risikoanalyse (Estimation of the production-related quality and service
life of asphalt wearing courses with the aid of risk analysis). Technischen Universität Darmstadt, 2010
Stichting Bouwkwaliteit (SBK) – Foundation for Building Quality; “Determination Method: Environ-
mental Performance of Buildings and Civil Engineering Works”
Stichting Nationale Milieudatabase; Bepalingsmethode Milieuprestatie Bouwwerken; Version 1.0;
July 2020; Berekeningswijze voor het bepalen van de milieuprestatie van bouwwerken ge-durende
hun gehele levensduur, gebaseerd op de EN 15804.
Windbranche.de – Das Branchenportal rund um die Windenergie. Wind power and electricity gene-
ra-tion in Great Britain: https://www.windbranche.de/wind/windstrom/windenergie-grossbritan-
nien, last accessed 19 July 2021.
Standards and laws
ISO 14040:2006, Environmental management - Life cycle assessment - Principles and framework
ISO 14044:2006, Environmental management - Life cycle assessment - Requirements and guidelines
ISO 14025:2006: Environmental labels and declarations — Type III environmental declarations — Prin-
ciples and procedures EN 13249
EN 15804:2012+A2:2019 Sustainability of construction works — Environmental Product Declarations
— Core rules for the product category of construction products
PCR A: General Program Category Rules for Construction Products from the EPD program Kiwa-Ecobil-
ity Experts, R.0_2021-07-16
PCR B: Product Category Rules (PCR) from the Kiwa-Ecobility Experts EPD program: “Geosynthetic
products”, edition 2022-02-08 (draft)
Page | 14 Tensar International Limited – Tensar® TriAx® TX150L-GD
Publisher Mail DE.Ecobility.Ex-
Kiwa-Ecobility Experts perts@kiwa.com
Voltastr. 5 Web https://www.kiwa.com/de/
13355 Berlin de/themes/ecobility-ex-
Germany perts/ecobility-experts/
Programme operator Mail DE.Ecobility.Ex-
Kiwa-Ecobility Experts perts@kiwa.com
Voltastr. 5 Web https://www.kiwa.com/de/
13355 Berlin de/uber-kiwa/ecobility-ex-
Germany perts/
Author of the Life Cycle Tel. +49 (0)30 467761-43
Assessment Fax. +49 (0)30 467761-10
Kiwa-Ecobility Experts Mail DE.Ecobility.Ex-
Voltastr.5 perts@kiwa.com
13355 Berlin Web https://www.kiwa.com/
Germany
Owner of the declaration Tel. +44 (0)1254 262 431
Tensar International Limited Fax. +44 (0) 1254 266 867
Units 2-4 Cunningham Court Mail info@tensar-internatio-
Shadsworth Business Park nal.com
Blackburn, United Kingdom Web www.tensar.co.uk
Page | 15 Tensar International Limited – Tensar® TriAx® TX150L-GD
