ENVIRONMENTAL PRODUCT DECLARATION
as per ISO 14025 and EN 15804+A2
Owner of the Declaration Knauf Ceiling Solutions GmbH & Co. KG
Publisher Institut Bauen und Umwelt e.V. (IBU)
Programme holder Institut Bauen und Umwelt e.V. (IBU)
Declaration number EPD-KNA-20230155-IBA1-EN
Issue date 15.08.2023
Valid to 14.08.2028
TOPIQ Prime – Tegular
Knauf Ceiling Solutions GmbH & Co. KG
www.ibu-epd.com | https://epd-online.com
1. General Information
Knauf Ceiling Solutions GmbH & Co. KG TOPIQ Prime – Tegular
Programme holder Owner of the declaration
IBU – Institut Bauen und Umwelt e.V. Knauf Ceiling Solutions GmbH & Co. KG
Hegelplatz 1 Elsenthal 15
10117 Berlin 94481 Grafenau
Germany Germany
Declaration number Declared product / declared unit
EPD-KNA-20230155-IBA1-EN 1 m² TOPIQ Prime - Tegular tiles with a surface weight of 2.49 kg/m².
This declaration is based on the product category rules: Scope:
Mineral panels, 01.08.2021 This document refers to 1 m² TOPIQ Prime - Tegular tiles with a surface
(PCR checked and approved by the SVR) weight of 2.49 kg/m², manufactured at the production facility in Grafenau,
Germany.
Issue date The owner of the declaration shall be liable for the underlying information
and evidence; the IBU shall not be liable with respect to manufacturer
15.08.2023
information, life cycle assessment data and evidences.
The EPD was created according to the specifications of EN 15804+A2. In
Valid to
the following, the standard will be simplified as EN 15804.
14.08.2028
Verification
The standard EN 15804 serves as the core PCR
Independent verification of the declaration and data according to ISO
14025:2011
internally X externally
Dipl.-Ing. Hans Peters
(Chairman of Institut Bauen und Umwelt e.V.)
Florian Pronold Matthias Schulz,
(Managing Director Institut Bauen und Umwelt e.V.) (Independent verifier)
1 Environmental Product Declaration - Knauf Ceiling Solutions GmbH & Co. KG - TOPIQ Prime – Tegular
2. Product
exceeding 0.1 percentage by mass: No
2.1 Product description/Product definition
The ceiling tiles consist of mineral wool (rock wool) and a This product/article/at least one partial article contains other
phenolic binder. The soft mineral tiles meet the requirements of carcinogenic, mutagenic, reprotoxic (CMR) substances in
EN 13964. categories 1A or 1B which are not on the candidate list,
exceeding 0.1 percentage by mass: No
The TOPIQ Prime - Tegular soft mineral tiles are available in
different formats. Biocide products were added to this construction product or it
has been treated with biocide products (this then concerns a
For the placing on the market of the product in the European treated product as defined by the (EU) Ordinance on Biocide
Union/European Free Trade Association (EU/EFTA) (with the Products No. 528/2012): No
exception of Switzerland) Regulation (EU) No. 305/2011 (CPR)
applies. The product needs a declaration of performance taking 2.6 Manufacture
into consideration EN 13964:2014, suspended ceiling The raw boards for the TOPIQ soft mineral tiles are sourced
requirements and test methods and the CE-marking. For the from Knauf Insulation from the plant in Nová Baňa (Slovakia),
application and use the respective national provisions apply. see International EPD System EPD 2022.
2.2 Application In the Grafenau plant, the panels are laminated with a glass
Soft mineral tiles are typically used as lay-in for suspended fleece, cut to size and the edges are machined. The TOPIQ
ceiling constructions. They are primarily used as optical tiles are painted with dispersion paint.
cladding, but also for sound absorption and sound insulation,
for fire resistance and against fire spreading as well as for The Grafenau factory is certified according to ISO 9001, ISO
hygiene requirements. 14001, ISO 45001 and ISO 50001.
2.3 Technical Data 2.7 Environment and health during manufacturing
Soft Mineral boards are regulated by EN 13964 and have The manufacturer complies with the special German and
corresponding labelling and declaration of performance. The European regulations for the production of mineral slabs:
following data provide an overview of results:
• The manufacturing plant is certified according to ISO
Construction data (according to DIN 18177) 9001, ISO 14001, ISO 45001 and ISO 50001.
Name Value Unit • The production has a closed water cycle.
• Production generates virtually no waste, all resulting
Thermal conductivity 0.04 W/(mK)
blanks, dust and rejects are reused.
Sound absorption coefficient acc. ISO 354 and
0.95 % • Exclusive use of mineral fibres according to Regulation
ISO 11654
(EU) No.1272/2008 Note Q.
Airborne sound reduction acc. ISO 10848 and
13 dB • Prohibition of the production and use of biopersistent
EN 717-1
fibres (Ordinance on Hazardous Substances, Annexe II,
Gross density (of the raw board) 140 kg/m3 No. 5).
Formaldehyde emissions acc. EN 717-1 13 μg/m3 • Prohibition of placing biopersistent fibres on the market
(Chemicals Prohibition Ordinance, No.23 of the Annexe
Additional technical data are not relevant for this product. to §1).
• Not subject to declaration according to REACH.
Performance data of the product in accordance with the
declaration of performance with respect to its essential 2.8 Product processing/Installation
characteristics according to EN 13964:2014, suspended ceiling There are no recognised systemic hazards associated with the
requirements and test methods (not part of CE-marking). installation of ceiling tiles. It is recommended that materials are
handled in a manner that minimises dust generation. Workers
2.4 Delivery status
should wear appropriate personal protective equipment.
The EPD refers to tiles with a thickness of 15 mm which can Equipment such as gloves, goggles and dust masks are
have variable length and width dimensions. recommended to minimise exposure to dust and prevent skin
irritation.
2.5 Base materials/Ancillary materials
Mineral tile composition: 2.9 Packaging
The panels are packaged in cardboard boxes and sealed with
Name Value Unit
transparent polyethylene film. These packages lie on
Basalt 46-51 %
chemically untreated wooden pallets. The pallets are wrapped
Dolomite - Limestone 13-17 % with polyethylene stretch film. Foil, paper and wood can be
Recovered metallurgical slags 25 % recycled in the usual ways.
Thermo set resin binder 2-4 %
2.10 Condition of use
Additives < 1 %
When handled properly, the mechanical and structural-physical
Fleece 7 %
properties of the soft mineral tile remain intact throughout its
Glue application rate 3 % entire service life.
Finish 6 %
2.11 Environment and health during use
The recycled content is at least 28 %.
When properly installed, no dust/particles are released during
the use phase. For the substance groups formaldehyde, volatile
This product/article/at least one partial article contains
organic compounds (VOCs) and total volatile organic
substances listed in the ECHA-candidate list (date: 25.06.2020)
2 Environmental Product Declaration - Knauf Ceiling Solutions GmbH & Co. KG - TOPIQ Prime – Tegular
compounds (TVOCs), the limits according to DIN 18177 are treatment plant, they are biodegradable, increasing the
complied with. chemical oxygen demand (COD) and biological oxygen
demand (BOD).
2.12 Reference service life
The service life of the soft mineral tiles is up to 50 years, Mechanical destruction
depending on the area of use, exposure and state of The soft mineral tiles can be broken by hand and also damaged
maintenance. Within the framework of the conditions of use, no superficially, which can result in minor dust formation.
ageing effects are to be expected apart from visual
discolouration caused by air circulation. 2.14 Re-use phase
If the panels are removed properly, they can be reinstalled. In
2.13 Extraordinary effects case of minor damage, the slabs can be reused as cut-to-size
Fire tiles. Mineral tiles can be returned to the manufacturing process
The declared products are classified in the fire reaction class if they are of the correct type and have sufficient material
A1 according to EN 13501-1. This means that they are "non- quality; they can be recycled up to 100 %.
combustible" according to the German building authority
designation (and also many other European countries). 2.15 Disposal
The waste code number of production residues for mineral tiles
Fire Reaction
according to the AVV, German List of Wastes Ordinance is 10
Name Value
11 03, the waste code number for construction site waste
Building material class A1 (offcuts) is 17 06 04. If the tiles are not recycled as described in
Smoke gas development - 2.14., they are disposed of in a landfill.
Burning droplets -
2.16 Further information
Further information at www.knaufceilingsolutions.com
Water DoPs at https://downloads.knaufceilingsolutions.com
Prolonged contact with water, can lead to a loss of structure,
and if the soluble components are discharged into the sewage
3. LCA: Calculation rules
3.1 Declared Unit Modul C2 | Transport to disposal
This EPD refers to a declared unit of 1 m² TOPIQ Prime - The transport to the disposal of the material is estimated
Tegular panels with a surface weight of 2.49 kg/m² and a declaring a 50 km radius to the landfill. In reality, this scenario
thickness of 15 mm. may vary depending on the actual location of deconstruction
Declared unit and referring waste treatment.
Name Value Unit
Module C3 | Waste processing
Declared unit 1 m2 The declared scenario assumes landfilling of the product.
Grammage 2.49 kg/m2 Referring environmental impacts are accounted for in module
Layer thickness 0.015 m C4.
The panels are produced at the Knauf Ceiling Solutions
Module C4 | Disposal
production site in Grafenau, Germany under the brand name
Module C4 refers to the emissions from the disposal of the
TOPIQ.
stone wool panels. The chosen scenario, therefore, includes
Various types of panels are produced at the site. A
the environmental burdens of landfilling of the product.
differentiation between the product groups was made based on
the recipe of the products.
Module D | Benefits and loads beyond the system
boundary
3.2 System boundary
The declared scenario assumes landfilling of the product.
The life cycle assessment of TOPIQ panels includes a cradle-
Referring environmental impacts are accounted for in module
to-gate analysis of the products' environmental impacts with
C4. There are no benefits and loads in module D.
modules (A1–A3, +C, +D). Subsequent life cycle phases are
part of the analysis: 3.3 Estimates and assumptions
Assumptions and approximations are applied in case of a lack
Module A1–A3 | Production stage
of representative data. All assumptions and approximations are
The production stage includes the upstream burdens of raw
documented precisely and represent a best-guess
material supply, their transports and the manufacturing
representation of reality. In case of uncertainty, a conservative
processes of the panels at the plant of Knauf Ceiling Solutions
approach is chosen.
located in Grafenau (Germany). Stone wool panels are coated
on site. Main raw material inputs, therefore, refer to stone wool 3.4 Cut-off criteria
panels, fleece and adhesive. The production site is supplied The LCA model covers all available input and output flows,
with electricity from the German power grid and thermal energy which can be represented based on robust data. Data gaps are
from natural gas. Also, the packaging of the products is filled with conservative assumptions from average data (when
considered. available) or with generic data and are documented
accordingly. Only data with a contribution lower than 1 % were
Module C1 | Deconstruction and demolition cut off. Thus, no data were neglected, of which a substantial
Disassembly of the product is done either manually or using impact is to be expected. All relevant data were collected
smaller tools. The referring energy demand is considered to be comprehensively. Cut-off material and energy flows were
negligible. chosen carefully based on their expected quantitative
contribution as well as potential environmental impacts. Thus, it
3 Environmental Product Declaration - Knauf Ceiling Solutions GmbH & Co. KG - TOPIQ Prime – Tegular
can be assumed that the sum of all neglected input flows does
not account for more than 5 % of the total material, water and 3.7 Period under review
energy flows. Foreground data were collected in the 2022 production year,
and the data are based on the volumes produced on an annual
3.5 Background data basis.
This study uses generic background data for the evaluation of
upstream environmental impacts from GaBi databases (GaBi 3.8 Geographic Representativeness
10; 2022.2). Land or region, in which the declared product system is
manufactured, used or handled at the end of the product´s
lifespan: Germany
3.6 Data quality
Data collection is based on product-specific questionnaires. It
3.9 Allocation
follows an iterative process of clarifying questions via e-mail,
telephone calls or in personal/web meetings. Intensive All information for the allocation of given material and energy
discussions between Knauf Ceiling Solutions and Daxner & flows is based on the Enterprise Resource Planning (ERP)-
Merl result in an accurate mapping of product-related material systems of the production site. Product-specific application
and energy flows. This leads to a high quality of foreground rates of finish, adhesive and glass fleece were provided by the
data collected. Data collection relies on a consistent process manufacturer. Furthermore, product-specific input rates for
according to ISO 14044. electric and thermal energy as well as the material efficiency
during production were provided by Knauf Ceiling Solutions.
The technological, geographical and time-related
3.10 Comparability
representativeness of the database was kept in mind when
Basically, a comparison or an evaluation of EPD data is only
selecting background data. Whenever specific data were
possible if all the data sets to be compared were created
missing, either generic datasets or representative average data
according to EN 15804 and the building context, respectively
were used instead. The implemented GaBi background
the product-specific characteristics of performance, are taken
datasets refer to the latest versions available (not more than
into account.
ten years old) and are carefully chosen. n-butyl acrylate
represents an exception to this rule tracing back to the
The GaBi background database was used to calculate the LCA
reference year of 2012. Due to a lack of other, more actual data
(GaBi 10; 2022.2).
and its minor influence on the results, this dataset was deemed
as a suitable approximation for this assessment.
4. LCA: Scenarios and additional technical information
Characteristic product properties of biogenic carbon
The declared product does not contain any biogenic carbon.
Information on the description of the biogenic carbon Assembly (A5)
content at the factory gate The End-of-Life of the product packaging is not declared in
Name ValueUnit module A5.
kg Name Value Unit
Biogenic carbon content in product -
C Packaging (cardboard) 0.047 kg/m²
Biogenic carbon content in accompanying 0.08 kg Packaging (pallets) 0.127 kg/m²
packaging C
Packaging (polyethylene-film) 0.0142 kg/m²
The carbon stored in the packaging was taken into account as
"CO -neutral". Thus the storage effect of the carbon bound in
2
End-of-Life (C1–C4)
the packaging is not included in the calculation but is
considered as emitted immediately. Name Value Unit
Collected separately 2.49 kg
Landfilling 2.49 kg
4 Environmental Product Declaration - Knauf Ceiling Solutions GmbH & Co. KG - TOPIQ Prime – Tegular
5. LCA: Results
The following table contains the LCA results for a declared unit of 1 m² TOPIQ Prime - Tegular panels with a surface weight of
2.49 kg/m² and a thickness of 15 mm.
DESCRIPTION OF THE SYSTEM BOUNDARY (X = INCLUDED IN LCA; ND = MODULE OR INDICATOR NOT DECLARED; MNR =
MODULE NOT RELEVANT)
Benefits and
Construction loads beyond
Product stage Use stage End of life stage
process stage the system
boundaries
la ire ta m w a Ry lp p u s tro p s n a rT g n iru tc a fu n a M e h t m o rf tro p s n a rTe tis e h t o t e ta g y lb m e s s A e s U e c n a n e tn ia M ria p e R tn e m e c a lp e R tn e m h s ib ru fe R y g re n e la n o ita re p Oe s u re ta w la n o ita re p Oe s u n o itc u rts n o c -e Dn o itilo m e d tro p s n a rT g n is s e c o rp e ts a W la s o p s iD -e s u e R-y re v o c e R-g n ilc y c e Rla itn e to p
A1 A2 A3 A4 A5 B1 B2 B3 B4 B5 B6 B7 C1 C2 C3 C4 D
X X X MND MND MND MND MNR MNR MNR MND MND X X X X X
RESULTS OF THE LCA - ENVIRONMENTAL IMPACT according to EN 15804+A2: 1 m² TOPIQ Prime - Tegular panels (2.49
kg/m²)
Parameter Unit A1-A3 C1 C2 C3 C4 D
Global Warming Potential total (GWP-total) kg CO 2 eq 3.75E+00 0 7.55E-03 0 3.62E-02 0
Global Warming Potential fossil fuels (GWP-fossil) kg CO 2 eq 4.08E+00 0 7.5E-03 0 3.72E-02 0
Global Warming Potential biogenic (GWP-biogenic) kg CO 2 eq -3.39E-01 0 0 0 -1.1E-03 0
Global Warming Potential luluc (GWP-luluc) kg CO 2 eq 1.81E-03 0 5.04E-05 0 6.87E-05 0
Depletion potential of the stratospheric ozone layer (ODP) kg CFC11 eq 1.11E-11 0 7.35E-16 0 8.74E-14 0
Acidification potential of land and water (AP) mol H+ eq 3.23E-02 0 2.5E-05 0 2.64E-04 0
Eutrophication potential aquatic freshwater (EP-freshwater) kg P eq 5.7E-06 0 2.67E-08 0 6.31E-08 0
Eutrophication potential aquatic marine (EP-marine) kg N eq 2.63E-03 0 1.14E-05 0 6.74E-05 0
Eutrophication potential terrestrial (EP-terrestrial) mol N eq 2.9E-02 0 1.28E-04 0 7.41E-04 0
Formation potential of tropospheric ozone photochemical oxidants kg NMVOC
9.07E-03 0 2.24E-05 0 2.05E-04 0
(POCP) eq
Abiotic depletion potential for non fossil resources (ADPE) kg Sb eq 6.16E-07 0 7.54E-10 0 3.81E-09 0
Abiotic depletion potential for fossil resources (ADPF) MJ 6.15E+01 0 9.82E-02 0 4.87E-01 0
m3 world eq
Water use (WDP) 2.09E-01 0 8.37E-05 0 4.08E-03 0
deprived
RESULTS OF THE LCA - INDICATORS TO DESCRIBE RESOURCE USE according to EN 15804+A2: 1 m² TOPIQ Prime - Tegular
panels (2.49 kg/m²)
Parameter Unit A1-A3 C1 C2 C3 C4 D
Renewable primary energy as energy carrier (PERE) MJ 5.8E+00 0 6.81E-03 0 7.31E-02 0
Renewable primary energy resources as material utilization
MJ 5.31E+00 0 0 0 0 0
(PERM)
Total use of renewable primary energy resources (PERT) MJ 1.11E+01 0 6.81E-03 0 7.31E-02 0
Non renewable primary energy as energy carrier (PENRE) MJ 5.89E+01 0 9.86E-02 0 4.88E-01 0
Non renewable primary energy as material utilization (PENRM) MJ 2.65E+00 0 0 0 0 0
Total use of non renewable primary energy resources (PENRT) MJ 6.16E+01 0 9.86E-02 0 4.88E-01 0
Use of secondary material (SM) kg 7.51E-01 0 0 0 0 0
Use of renewable secondary fuels (RSF) MJ 0 0 0 0 0 0
Use of non renewable secondary fuels (NRSF) MJ 0 0 0 0 0 0
Use of net fresh water (FW) m3 1.19E-02 0 7.87E-06 0 1.24E-04 0
RESULTS OF THE LCA – WASTE CATEGORIES AND OUTPUT FLOWS according to EN 15804+A2:
1 m² TOPIQ Prime - Tegular panels (2.49 kg/m²)
Parameter Unit A1-A3 C1 C2 C3 C4 D
Hazardous waste disposed (HWD) kg 9.43E-07 0 5.22E-13 0 2.51E-11 0
Non hazardous waste disposed (NHWD) kg 6.62E-01 0 1.61E-05 0 2.5E+00 0
Radioactive waste disposed (RWD) kg 2.64E-03 0 1.83E-07 0 5.42E-06 0
Components for re-use (CRU) kg 0 0 0 0 0 0
Materials for recycling (MFR) kg 0 0 0 0 0 0
Materials for energy recovery (MER) kg 0 0 0 0 0 0
Exported electrical energy (EEE) MJ 0 0 0 0 0 0
Exported thermal energy (EET) MJ 0 0 0 0 0 0
RESULTS OF THE LCA – additional impact categories according to EN 15804+A2-optional:
1 m² TOPIQ Prime - Tegular panels (2.49 kg/m²)
Parameter Unit A1-A3 C1 C2 C3 C4 D
5 Environmental Product Declaration - Knauf Ceiling Solutions GmbH & Co. KG - TOPIQ Prime – Tegular
Disease
Incidence of disease due to PM emissions (PM) 2.74E-07 0 1.43E-10 0 3.25E-09 0
incidence
Human exposure efficiency relative to U235 (IR) kBq U235 eq 2.04E-01 0 2.76E-05 0 6.02E-04 0
Comparative toxic unit for ecosystems (ETP-fw) CTUe 1.79E+01 0 6.96E-02 0 2.73E-01 0
Comparative toxic unit for humans (carcinogenic) (HTP-c) CTUh 8.05E-10 0 1.43E-12 0 4.17E-11 0
Comparative toxic unit for humans (noncarcinogenic) (HTP-nc) CTUh 3.24E-08 0 8.8E-11 0 4.61E-09 0
Soil quality index (SQP) SQP 1.08E+02 0 4.16E-02 0 1.01E-01 0
Disclaimer 1 – for the indicator 'Potential Human exposure efficiency relative to U235'.
This impact category deals mainly with the eventual impact of low dose ionizing radiation on human health of the nuclear fuel cycle. It
does not consider effects due to possible nuclear accidents, occupational exposure nor due to radioactive waste disposal in
underground facilities. Potential ionizing radiation from the soil, from radon and from some construction materials is also not measured
by this indicator. Disclaimer 2 – for the indicators 'abiotic depletion potential for non-fossil resources', 'abiotic depletion potential for
fossil resources', 'water (user) deprivation potential, deprivation-weighted water consumption', 'potential comparative toxic unit for
ecosystems', 'potential comparative toxic unit for humans – cancerogenic', 'Potential comparative toxic unit for humans - not
cancerogenic', 'potential soil quality index'.
The results of this environmental impact indicator shall be used with care as the uncertainties on these results are high or as there is
limited experienced with the indicator.
6. LCA: Interpretation
The following interpretation contains a summary of the LCA Tegular panels.
results referenced to a declared unit of 1 m² TOPIQ Prime -
The comparison of the product's life cycle phases shows a especially electricity, has an influence on the potential climate
clear dominance of the production phase (modules A1–A3) in change (GWP), as well as depletion of fossil resources (ADPF).
all environmental impact categories. The potential
environmental impacts from transport to disposal (module C2) The emissions of biogenic greenhouse gases (GWP-biogenic)
and the End-of-Life of the products due to landfilling (module originate from the packaging of the rock mineral wool raw
C4) have a minor contribution. boards that is included in the used EPD results as well as the
packaging of the TOPIQ panels.
The environmental effects in the production phase are mainly Greenhouse-gas emissions from land use change (GWP luluc)
dominated by the supply chain of the purchased rock mineral result apart from the upstream supply chain of rock mineral
wool boards in all categories considered. As the representation wool boards, from transport as well as packaging. When it
of the upstream footprint of the raw board is based on a comes to the eutrophication potential of freshwater (EP-
product-specific EPD, a high quality of the results is to be freshwater), also packaging has a dominant role.
expected. Abiotic depletion potential for non-fossil resources (ADPE) is
Furthermore, the supply chain of purchased energy carriers, also influenced by the top coat as well as the adhesive system.
6 Environmental Product Declaration - Knauf Ceiling Solutions GmbH & Co. KG - TOPIQ Prime – Tegular
7. Requisite evidence
Number: 392-2022-00122903_A_EN
7.1 Radioactivity Testing period: 15.09.2022-13.10.2022
Measurements of radioactivity did not reveal any evidence of Test basis: ISO 16000-6
artificial radioactivity outside the natural background radiation.
AgBB Overview (28 days)
Measuring point: TÜV Süd Industrie Service
Name Value Unit
Test Number: G 7141 002
Testing Date: 14.12.2016 TVOC (C6 - C16) < 5 μg/m3
Sum SVOC (C16 - C22) < 5 μg/m3
7.2 Biopersistence R (dimensionless) 0.13 -
The mineral wool used for the production of the panels is
VOC without NIK < 5 μg/m3
biosoluble and, according to EU Regulation 1272/2008/EC, is
Carcinogenic substances < 1 μg/m3
to be assessed as free of suspected cancer. The "RAL Mineral
Wool Quality Seal" monitors and guarantees the quality of the
AgBB Overview (3 days)
wool used.
Name Value Unit
The production and use of non-exempt fibres is prohibited by
the Ordinance on Hazardous Substances and the Chemicals TVOC (C6 - C16) 25 μg/m³
Prohibition Ordinance. Sum SVOC (C16 - C22) < 5 μg/m³
R (dimensionless) 0.43 -
7.3 VOC emissions
VOC without NIK < 5 μg/m³
Measuring point: Eurofins Product Testing A/S
Carcinogenic Substances < 1 μg/m³
Test report: VOC emission test report Indoor Air Comfort GOLD
(10.11.2022)
8. References
Standards ISO 11654
DIN EN ISO 11654:1997-07, Acoustics - Sound absorbers for
DIN 18177 use in buildings - Evaluation of sound absorption.
DIN 18177:2020-12, Wet-felt factory-produced mineral panels.
ISO 14001
EN 13501-1 DIN EN ISO 14001:2015-11, Environmental management
DIN EN 13501-1:2019, Classification of construction products systems - Requirements with guidance for use.
and building elements according to their reaction to fire, Part 1:
Classification with the results of tests on the reaction to fire of ISO 14025
construction products. DIN EN ISO 14025:2011-10, Environmental labels and
declarations — Type III environmental
EN 13964 declarations — Principles and procedures.
DIN EN 13964:2014, Suspended ceilings - Requirements and
test methods. ISO 14044
DIN EN ISO 14044:2006-10, Environmental management – Life
EN 15804 cycle assessment – Requirements and guidelines.
DIN EN 15804:2012+A2:2019+AC:2021, Sustainability of
construction works - Environmental product declarations - Core ISO 16000-6
rules for the product category of construction products. ISO 16000-6:2011-12, Indoor air contaminants - Part 6:
Determination of VOCs in indoor air and test chambers,
EN 16487 sampling on Tenax TA®, thermal desorption and gas
DIN EN 16487:2015-02, Acoustics - Test specifications for chromatography with MS/FID.
suspended ceilings - Sound absorption.
ISO 45001
ISO 354 DIN ISO 45001:2018-06, Occupational health and safety
DIN EN ISO 354:2003-12, Acoustics - Measurement of sound management systems - Requirements withguidance for use.
absorption in reverberant rooms.
ISO 50001
ISO 717-1 DIN EN ISO 50001:2011-12, Energy management systems -
DIN EN ISO 717-1:2013-06, Acoustics - Assessment of sound Requirements with guidance for use.
insulation in buildings and of building elements - Part 1:
Airborne sound insulation. Further References
ISO 9001 AgBB
DIN EN ISO 9001:2015-11, Quality management systems - Ausschuss zur gesundheitlichen Bewertung von Bauprodukte
Requirements. (AgBB) (Committee for health-related evaluation of building
products): Vorgehensweise bei der gesundheitlichen
ISO 10848 Bewertung der Emissionen von flüchtigen organischen
DIN EN ISO 10848:2006-08, Acoustics - Measurement of Verbindungen (VOC und SVOC) aus Bauprodukten.
airborne and impact sound transmission between adjacent
rooms in test stands. AVV, German List of Wastes Ordinance
Regulation on the European Waste List.
7 Environmental Product Declaration - Knauf Ceiling Solutions GmbH & Co. KG - TOPIQ Prime – Tegular
Chemicals Prohibition Ordinance PCR Part A
Chemicals Prohibition Ordinance (Germandesignation: Product category rules for building-related products and
Chemikalien-Verbotsverordnung – ChemVerbotsV) of 20 services. Part A: Calculation rules for the life cycle assessment
January 2017 (Federal LawGazette I p. 94; 2018 I p. 1389), last and requirements on the project report according to
amended by Article 300 of the Ordinance of 19 June 2020 EN15804+A2:2019. Version 1.3, Berlin: Institut Bauen und
(Federal Law Gazette I p. 1328). Umwelt e.V. (Hrsg.), 2022.
ECHA-candidate list PCR: Mineral panels
List of substances of very high concern (SVHC) for Institut Bauen und Umwelt e.V. (IBU), 2023. Product Category
authorisation (ECHA Candidate List), 25.06.2020, published Rules for Building-Related Products and Services. Part B:
under Article 59(10) of REACH. Helsinki: European Chemicals Requirements on the EPD for Mineral panels. Version v2,
Agency. 31.05.2023.
Eurofins Product Testing A/S RAL Mineral Wool Quality Seal
Test report: VOC emission test report Indoor Air Comfort GOLD GGM members with the right to use the RAL quality mark
(10.11.2022), Number: 392-2022-00122903_A_EN. including plants and fibre types, as of January 2021.
GaBi REACH
GaBi 10, Software-System and Database for Life Cycle Regulation (EC) No 1907/2006 of the European Parliament and
Engineering. DB 2022.2. Sphera, 1992-2022. Available at: Council from 18 December 2006, Regulation concerning the
https://sphera.com/product-sustainability-gabi-data-search/. Registration, Evaluation, Authorisation and Restriction of
Chemicals (REACH).
IBU 2021
Institut Bauen und Umwelt e.V.: General instructions for the Regulation (EU) Nr. 305/2011(CPR)
EPD programme of Institut Bauen und Umwelt e.V. (IBU). Regulation (EU) No 305/2011 of the European Parliament and
Version 2.0, Berlin: Institut Bauen und Umwelt e.V., 2021. of the Council of 9 March 2011 laying down harmonised
www.ibuepd.com conditions for the marketing of construction products and
repealing Council Directive 89/106/EEC Text with EEA
International EPD System EPD 2022 relevance.
Environmental poduct declaration in accordance with ISO
14025, ISO 21930 and EN 15804+A2: PTN, TP from Knauf Regulation (EU) Nr.1272/2008
Insulation Sprl. EPD registration number: S-P-05553, 2022. Regulation (EC) No 1272/2008 of the European Parliament and
of the Council of 16 December 2008 on classification, labelling
Ordinance on Biocide Products and packaging of substances and mixtures, amending and
Regulation (EU) No 528/2012 of the European Parliament and repealing Directives 67/548/EEC and 1999/45/EC, and
of the Council of 22 May 2012 concerning the making available amending Regulation (EC) No 1907/2006.
on the market and use of biocidal products.
TÜV Süd Industrie Service
Ordinance on Hazardous Substances TÜV Strahlenmesslabor. IS-ETS1-MUC/er.
Ordinance on Hazardous Substances, of 26 November 2010
(Federal Law Gazette I p. 1643, 1644), last amended by Article
148 of the Law of 29 March 2017 (Federal Law Gazette I p.
626).
8 Environmental Product Declaration - Knauf Ceiling Solutions GmbH & Co. KG - TOPIQ Prime – Tegular
Publisher
Institut Bauen und Umwelt e.V. +49 (0)30 3087748- 0
Hegelplatz 1 info@ibu-epd.com
10117 Berlin www.ibu-epd.com
Germany
Programme holder
Institut Bauen und Umwelt e.V. +49 (0)30 3087748- 0
Hegelplatz 1 info@ibu-epd.com
10117 Berlin www.ibu-epd.com
Germany
Author of the Life Cycle Assessment
Daxner & Merl GmbH +43 676 849477826
Lindengasse 39/8 office@daxner-merl.com
1070 Wien www.daxner-merl.com
Austria
Owner of the Declaration
Knauf Ceiling Solutions GmbH & Co. KG 0049 8552 422 0
Elsenthal 15 info@knaufamf.com
94481 Grafenau www.knaufceilingsolutions.com
Germany
9 Environmental Product Declaration - Knauf Ceiling Solutions GmbH & Co. KG - TOPIQ Prime – Tegular
