ENVIRONMENTAL PRODUCT DECLARATION
as per ISO 14025 and EN 15804+A1
Owner of the Declaration Troldtekt A/S
Programme holder Institut Bauen und Umwelt e.V. (IBU)
Publisher Institut Bauen und Umwelt e.V. (IBU)
Declaration number EPD-TRO-20220045-ICA1-EN
Issue date 07.04.2022
Valid to 06.04.2027
Acoustic panels - painted
Troldtekt A2 25 mm Natural Grey
based on FUTURECEM
www.ibu-epd.com | https://epd-online.com
Umwelt Produktdeklaration Name des Herstellers – Name des Produkts
1. General Information
Troldtekt A/S Troldtekt A2 25 mm Natural Grey
based on FUTURECEM - painted
Programme holder Owner of the declaration
IBU – Institut Bauen und Umwelt e.V. Troldtekt A/S
Panoramastr. 1 Sletvej 2 A
10178 Berlin 8310 Tranbjerg
Germany Denmark
Declaration number Declared product / declared unit
EPD-TRO-20220045-ICA1-EN Acoustic panel "A2 Natural Grey FUTURECEM" - 1 m2,
25 mm thickness - painted finish
This declaration is based on the product Scope:
category rules: This declaration represents the production, supply,
Wood cement - Mineral-bonded wooden composites, mounting, use, dismantling and disposal of 1 m2 (25
01.2019 mm thickness) of grey composite cement-bonded
(PCR checked and approved by the SVR) wood wool acoustic panel "A2 Natural Grey
FUTURECEM" with a painted finish, produced by
Troldtekt A/S, with a reference service life of 50 years.
Issue date
The production facility is located in Jutland, Denmark.
07.04.2022
Three scenarios represent its use in indoor conditions
in Denmark, Sweden and Germany.
Valid to
06.04.2027
The owner of the declaration shall be liable for the
underlying information and evidence; the IBU shall not
be liable with respect to manufacturer information, life
cycle assessment data and evidences.
The EPD was created according to the specifications
of EN 15804+A1. In the following, the standard will be
simplified as EN 15804.
Verification
The standard EN 15804 serves as the core PCR
Independent verification of the declaration and data
according to ISO 14025:2010
Dipl. Ing. Hans Peters internally x externally
(chairman of Institut Bauen und Umwelt e.V.)
Dr. Alexander Röder Ms Jane Anderson
(Managing Director Institut Bauen und Umwelt e.V.)) (Independent verifier)
2. Product
2.1 Product description/Product definition For the application and use, the respective national
Troldtekt A2 Natural Grey FUTURECEM acoustic provisions apply.
panels are some of the leading and preferred solutions
for creating a good indoor sound environment. They 2.2 Application
are sold in various thicknesses (20-35 mm) and The panels are installed on the ceilings and walls in
dimensions (width: 600 mm, lengths: 600/1200/2400 offices, businesses, schools, institutions, cultural sites,
mm or width: 625 mm, lengths: 625/1250/2500 sports centres, swimming pools and private homes.
mm). The panels can be unpainted or painted in a
wide variety of colours. 2.3 Technical Data
The table below indicates the technical specifications
For the placing on the market of the product in the of the panels in accordance with EN 13168, the
European Union/European Free Trade Association standard for cement-bonded wood wool and double-
(EU/EFTA) (with the exception of Switzerland) layer panels with cement-bonded wood wool, and EN
Regulation (EU) No. 305/2011 applies. The product 13964, the standard for suspended ceilings.
needs a declaration of performance taking into
consideration EN 13964:2014, Suspended ceilings.
Requirements and test methods, and the CE-marking.
2 Environmental Product Declaration Troldtekt A/S – Troldtekt 25mm A2 Natural Grey FUTURECEM - painted
29 %. The wood is then shredded to produce wool.
The wood wool is mixed together with Portland
composite cement, water, and additives. The mixture is
cast and cured using a heat press and dried with a
Technical specifications of the product covered in biomass-fired oven. The cast panel is milled to remove
this EPD any material in excess and cut edges. After
Name Value Unit approximately 4 weeks of curing, the panel can be
Gross density 523 kg/m3 painted before being stored on a pallet and packaged
Grammage 13.06 kg/m2 to be transported to central distribution warehouses.
Thermal conductivity acc. to EN
0.076 W/(mK)
13168:2012+A1:2015 2.7 Environment and health during
Water vapour diffusion resistance manufacturing
- -
factor acc. to DIN 4108-4 Troldtekt is following its working environment closely.
Sound absorption coefficient (only Both the physical working environment and sickness
with reference to the - % absence are closely monitored. It is an ongoing
corresponding component design) process involving both leaders and factory workers.
Light reflection (measured by
DELTA Light and Optics 26.3 - 70.8 % 2.8 Product processing/Installation
Reaction to fire A2/s1/d0 Installation instructions are available here:
https://www.troldtekt.com/Installation
2.9 Packaging
Performance data of the product in accordance with
The product is packaged with polyethylene plastic film
the declaration of performance with respect to its
and cardboard. The packaging material can be easily
essential characteristics according to EN
sorted and treated in dedicated waste recycling
13168:2012+A1:2015, Thermal insulation products for
channels. The packaged product is delivered on a
buildings. Factory made wood wool (WW) products.
returnable wood pallet.
Specification, and EN 13964:2014, Suspended
ceilings. Requirements and test methods.
2.10 Condition of use
2.4 Delivery status
Conditions of use are detailed
The panel is usually distributed in length of 600,
here: https://www.troldtekt.com/Installation/Use_and_
1200 or 2400 mm by 600 mm width or in length of 625,
maintenance
1250 or 2500 mm by 625 mm width. It comes in
three thicknesses: 20, 25 and 35 mm. Additionally,
2.11 Environment and health during use
several density ranges are available: Coarse, Fine,
Environmental and ecotoxicity risks from exposure to
Ultra-Fine and Extreme-Fine causing different
Troldtekt panel products during use have been
densities (388-428 kg/m3). The panels are normally
assessed and found eligible to the following
delivered in packs of 80 units on pallets.
certification schemes:
2.5 Base materials/Ancillary materials  Finnish M1 classification
The composition of the finished product is a mix of  Danish Indoor Climate
limestone (19.1 %), wood wool (23.2 %), Portland  Cradle to Cradle
composite cement (53.8 %), water (0.6 %), as well as
water glass (1.0 %) and accelerator (1,2 %).
These certificates can be accessed
Additionally, a painted finish is provided with a water-
here: https://www.troldtekt.com/Web-
based paint (1.1 %). The composition is at dry basis at
tools/Downloads/Certificates-and-tests
the factory gate, as most of the water has evaporated
during drying, but water remains bound to the wood
2.12 Reference service life
fibre and cement paste (hydrated cement).
The technical service life of the panel is superior to 50
years. This EPD refers to the service lifetime indicated
This product/article/at least one partial article contains
by the BBSR table for the material 353.311 of type
substances listed in the candidate list (date:
“Holzbekleidungen: Holz, Holzwerkstoff und
17.01.2022) exceeding 0.1 percentage by mass: No
Mehrschichtleichtbauplatten”.
This product/article/at least one partial article contains
Because the panel is used in a building, in this EPD its
other CMR substances in categories 1A or 1B which
reference service life is limited by the expected service
are not on the candidate list, exceeding 0.1 percentage
life of the building, which is commonly accepted as 50
by mass: No
years, at least as LCA timeframe.
Biocide products were added to this construction
There is no influence of the ageing of the material on
product or it has been treated with biocide products
its technical performance.
(this then concerns a treated product as defined by the
(EU) Ordinance on Biocide Products No. 528/2012):
2.13 Extraordinary effects
No
Fire
2.6 Manufacture
Information on the fire performance according to EN
Norway spruce logs from local forests (with a moisture
13168.
content of about 65-70 %) are received and the bark is
removed. The wood is stored for approximately six
Fire protection
months until the moisture content in the wood drops to
Name Value
3 Environmental Product Declaration Troldtekt A/S – Troldtekt 25mm A2 Natural Grey FUTURECEM - painted
Building material class A2
Burning droplets d0 2.15 Disposal
Smoke gas development s1 The product may be composted, thermally treated with
energy recovery, or landfilled.
Water
No information on the product performance under the European Waste Code: 10 13 11 (wastes from
unforeseeable influence of water is available. cement-based composite materials)
Mechanical destruction Painted panels must be incinerated at end-of-life.
No information on the product performance under
unforeseeable mechanical destruction is available. Additional information on disposal
options: https://www.troldtekt.com/environment-and-
2.14 Re-use phase csr/product-life-cycle/recycling/
Currently, Troldtekt panels undergo thermal treatment
with energy recovery. Composting is also possible. 2.16 Further information
For additional information on technical specifications,
Additional information on recycling you may consult the Declaration Of
options: https://www.troldtekt.com/~/media/Files/Info% Performance: https://www.troldtekt.com/Web-
20sheets/English/Troldtekt_Recycling%20instructions tools/Downloads/DoPs
%20pdf.pdf
3. LCA: Calculation rules
3.1 Declared Unit
The functional unit is 1 m2 of acoustic panel, in 25 mm 3.6 Data quality
thickness, corresponding to 13.06 kg of material with a Statistical representativeness
painted finish, mounted on the ceiling, with a reference The statistical representativeness of the product
service life of 50 years. system is very good. The input and output data
samples used to build inventories are based on the
Declared unit entirety of the annual production of panels in 2020 and
Name Value Unit is verified by a third party. Such representativeness is
Declared unit 1 m2 also valid for the production of Portland composite
Gross density 523 kg/m3 cement (FUTURECEM), whose EPD was published in
Grammage 13.06 kg/m2 2019 and audited in 2021. The EPD for the paint used
Layer thickness 0.025 m was published in 2018.
Temporal, geographical and technological
representativeness
3.2 System boundary All data strictly related to the cement production is
Cradle to grave technologically, temporally, and geographically
representative. The cement production data is less
3.3 Estimates and assumptions than 5 years old. The data used to model the
Assumptions are described occasionally throughout foreground inventory of acoustic panels dates from the
the section "LCA: Calculation rules". production year of 2020. As for secondary data, some
of the ecoinvent datasets are less than 3 years old.
3.4 Cut-off criteria
The cut-off criterion is applied according to EN 15804 3.7 Period under review
Section 6.3.5 and PCR part A Section 5.6. The primary data concerned with the manufacture (A1-
All inputs and outputs for which data are available are A3) relates to the production year 2020 and the data
included in the LCA model. Data gaps are filled with are based on the volumes produced on an annual
conservative assumptions from average data (when basis.
available) or with generic data and are documented
accordingly. 3.8 Allocation
The following product flows have been omitted Allocation of production data to the multiple produced
according to the 1 % cut-off rule: types of panels (with the same functional unit) is
 Wooden pallet to transport the product performed based on the rules provided in EN 15804.
Sub-processes associated to painting have especially
 Capital infrastructure (factory)
been allocated to the painted panels. Data such as
 Energy utilization of incinerated paint
waste generation and packaging have been allocated
 Allocation of burden from wood logging to to the entire production volume of panels in Troldtekt.
residual wood fractions The only case of co-produced outputs is associated to
wood logging. However, the environmental load is
evenly distributed over all its co-products, such as
logs, energy wood, and bark.
3.5 Background data
Two types of data source are used as secondary data:
3.9 Comparability
 Product-specific EPDs for the manufacture
Basically, a comparison or an evaluation of EPD data
and supply of Portland composite cement and is only possible if all the data sets to be compared
water-based paint were created according to EN 15804 and the building
 Database ecoinvent v.3.6 cut-off
4 Environmental Product Declaration Troldtekt A/S – Troldtekt 25mm A2 Natural Grey FUTURECEM - painted
context, respectively the product-specific The used background database is ecoinvent v.3.6 cut-
characteristics of performance, are taken into account. off
4. LCA: Scenarios and additional technical information
Manufacture (A1-A3) Capacity utilisation volume factor 1 -
Data
Primary data is third-party verified and based on the
production year 2020, within the facilities of Troldtekt
A/S in Jutland (Denmark).
Installation into the building (A5)
End-of-waste state and use of by-products Name Value Unit
For all processes supplying a residual material/waste Electricity consumption 0.060 kWh
that originates the end-of-life phase of a product to the Material loss (plastic film) 0.007 kg
product system to be used as input, the polluter-pay Material loss (cardboard) 0.032 kg
principle “100:0” is used. Some wooden by-products Use phase (B1)
generated during manufacture in Troldtekt end up as Before distribution and during the use phase (B1), the
soil improvers externally (reaching end-of-waste state), carbonation of the cement contained in the panel,
and thus their biogenic carbon leaves Troldtekt's during use, is accounted for. Based on laboratory
system boundary. measurement, the panel will absorb up to 140 grams of
carbon dioxide per kilogram of cement. Normalized to
Wind-certified electricity the reference flow, this corresponds to an uptake of
All the electricity used to produce the panels in Module approximately 0.7 kilograms of carbon dioxide by the
A3 originates from Danish wind power, for which a end of the service lifetime, including the uptake in A3.
certificate ensures the origin. It originates from a 1-3
MW offshore wind turbine, with transformation, Maintenance (B2)
transmission and distribution losses and is modelled As the panel does not require any maintenance except
correspondingly. for the occasional dusting, no maintenance module
(B2) is considered.
Carbon balance
Biogenic: Absorption of biogenic CO 2 by the purchased Maintenance (B2)
wood has been considered in A1. Some of it is As the panel does not require any maintenance except
released again during production in A3, some ends up for the occasional dusting, no maintenance module
sequestered in soil, while the majority of the remaining (B2) is considered.
biogenic CO , 6.10 kg, is retained in the finished
2
product and emitted during end-of-life incineration in
Name Value Unit
C4.
Fossil: Absorption of some fossil CO , originating from
2 Repair, replacement, refurbishment (B3, B4, B5)
the calcination of limestone during cement production,
As the technical service life of the panel is superior to
happens when the cement is mixed with water in A3. A
the assumed service life of the building (50 years), no
majority is absorbed during the use phase B1, and all
repair (B3), replacement (B4) or refurbishment (B5)
the absorbed fossil CO is finally emitted during end-
2 steps are considered.
of-life incineration in C4.
Distribution to site (A4) and mounting (A5) Name Value Unit
To consider the main geographical variants of the life
cycle of Troldtekt A2 Natural Grey FUTURECEM Replacement (B4) / Refurbishment (B5)
panels, three scenarios are developed, where the Name Value Unit
product is supplied, mounted, used and discarded in
Aarhus (Denmark), Hamburg (Germany) and Malmö Information about reference service life is detailed in
(Sweden). An additional 50 km from the local 2.12.
warehouse to construction site is assumed.
Reference service life
Name Value Unit
Transport to the building site (A4) Reference service life (according to 50 a
ISO 15686-1, -2, -7 and -8)
Name Value Unit
Litres of fuel 26.8 l/100km Life Span (according to BBSR) 50 a
Transport distance to Denmark 160 km Life Span according to the
75 a
Transport distance to Germany 370 km manufacturer
Transport distance to Sweden 394 km
Operational energy use (B6) and Operational water
Transport distance from
use (B7)
warehouse to local construction
sites in 50 km Name Value Unit
Water consumption - m3
Denmark/Germany/Sweden
Electricity consumption - kWh
Capacity utilisation (including
empty runs) 85 % Other energy carriers - MJ
Gross density of products Equipment output - kW
523 kg/m3
transported
5 Environmental Product Declaration Troldtekt A/S – Troldtekt 25mm A2 Natural Grey FUTURECEM - painted
End of life (C1-C4)
Name Value Unit
Electricity use (for un-mounting) 0.060 kWh
Transport (to material sorting
50 km
facility)
Collected as mixed construction
13.06 kg
waste
Energy recovery 2.99 kg
Energy recovery efficiency 10 %
Energy recovered 6.10 MJ
The panel is un-mounted at the end of its reference
service life and driven to the regional waste
incineration plant. Energy is recovered from the wood
part of the panel at 10 % efficiency.
Reuse, recovery and/or recycling potentials (D),
relevant scenario information
Name Value Unit
Electricity 1.45 MJ
Heat 4.65 MJ
The energy substituted from incineration of the panel's
wood component in C4 is considered to be a split of
the Danish electricity grid mix (for electricity) and
natural gas (for heat).
Details on possible disposal routes
Aalborg Portland cement factory utilizes dust and
offcuts from the Troldtekt factory as a raw material in
new cement, i.e. in the technical circle. During
incineration in the cement kiln, the wood content in the
cement-bonded wood wool panels replaces fossil
fuels, while the cement ends up as a raw material in
new cement, replacing virgin raw materials and heavy
fossil fuels, thereby avoiding a significant amount of
CO emissions. This scheme of wood wool waste as a
2
raw material can be scaled for construction site and
demolition waste. It will be gradually rolled out to all of
Denmark in the period 2021-2023. Once Denmark has
documented economic and environmental benefits to
be gained by including wood wool waste in the
production of new cement rather than going to waste
incineration or landfill, dialogue with municipalities and
local cement producers in the primary markets of
Troldtekt is initiated to facilitate similar schemes
regionally or nationally.
6 Environmental Product Declaration Troldtekt A/S – Troldtekt 25mm A2 Natural Grey FUTURECEM - painted
5. LCA: Results
Note: Global Warming Potential (GWP) indicator includes CO of both biogenic and fossil origin.
2
Also, GWP results for Troldtekt A2 Natural Grey FUTURECEM (painted) for other delivery scenarios in
respectively Germany and Sweden, are 2.58E-1 kg CO and 2.73E-1 kg CO .
2 2
DESCRIPTION OF THE SYSTEM BOUNDARY (X = INCLUDED IN LCA; MND = MODULE NOT DECLARED;
MNR = MODULE NOT RELEVANT)
BENEFITS AND
CONSTRUCTI LOADS
PRODUCT STAGE ON PROCESS USE STAGE END OF LIFE STAGE BEYOND THE
STAGE SYSTEM
BOUNDARIES
7 Environmental Product Declaration Troldtekt A/S – Troldtekt 25mm A2 Natural Grey FUTURECEM - painted
lairetam
waR
ylppus tropsnarT
gnirutcafunaM
eht
morf
tropsnarT
etis
eht
ot
etag
ylbmessA esU
ecnanetniaM
riapeR
tnemecalpeR tnemhsibrufeR
ygrene
lanoitarepO esu
retaw
lanoitarepO esu
noitcurtsnoc-eD
noitilomed tropsnarT
gnissecorp
etsaW
lasopsiD -esueR -yrevoceR -gnilcyceR laitnetop
A1 A2 A3 A4 A5 B1 B2 B3 B4 B5 B6 B7 C1 C2 C3 C4 D
X X X X X X MND MNR MNR MNR MND MND X X MND X X
RESULTS OF THE LCA - ENVIRONMENTAL IMPACT according to EN 15804+A1: 1 m2 A2 Natural Grey
FUTURECEM, 25 mm, painted finish, delivered and used in Denmark
Parameter Unit A1-A3 A4 A5 B1 C1 C2 C4 D
GWP [kg CO2-Eq.] 3.03E-1 1.29E-1 8.76E-2 -5.22E-1 6.50E-4 1.09E-1 6.80E+0 -7.98E-1
ODP [kg CFC11-Eq.] 2.64E-7 2.35E-8 1.64E-9 0.00E+0 2.81E-10 1.99E-8 5.36E-9 -4.41E-8
AP [kg SO2-Eq.] 1.85E-2 2.61E-4 5.90E-5 0.00E+0 1.59E-6 2.20E-4 4.43E-4 -1.66E-3
EP [kg (PO4)3--Eq.] 6.35E-3 5.36E-5 1.03E-4 0.00E+0 8.86E-7 4.53E-5 1.92E-4 -1.23E-3
POCP [kg ethene-Eq.] 1.02E-3 1.72E-5 2.58E-6 0.00E+0 8.88E-8 1.45E-5 3.47E-5 -9.52E-5
ADPE [kg Sb-Eq.] 7.80E-5 3.52E-6 2.09E-7 0.00E+0 1.82E-8 2.97E-6 5.84E-7 -2.14E-6
ADPF [MJ] 4.62E+1 1.96E+0 3.70E-1 0.00E+0 4.20E-2 1.66E+0 5.35E-1 -1.12E+1
GWP = Global warming potential; ODP = Depletion potential of the stratospheric ozone layer; AP = Acidification potential of land and water; EP =
Caption Eutrophication potential; POCP = Formation potential of tropospheric ozone photochemical oxidants; ADPE = Abiotic depletion potential for non-
fossil resources; ADPF = Abiotic depletion potential for fossil resources
RESULTS OF THE LCA - INDICATORS TO DESCRIBE RESOURCE USE according to EN 15804+A1: 1 m2
A2 Natural Grey FUTURECEM, 25 mm, painted finish, delivered and used in Denmark
Parameter Unit A1-A3 A4 A5 B1 C1 C2 C4 D
PERE [MJ] 6.05E+1 2.77E-2 1.60E-1 0.00E+0 3.91E-2 2.34E-2 7.06E+0 -5.22E+0
PERM [MJ] 6.15E+1 0.00E+0 0.00E+0 0.00E+0 0.00E+0 0.00E+0 0.00E+0 0.00E+0
PERT [MJ] 1.22E+2 2.77E-2 1.60E-1 0.00E+0 3.91E-2 2.34E-2 7.06E+0 -5.22E+0
PENRE [MJ] 5.79E+1 1.98E+0 4.58E-1 0.00E+0 4.31E-2 1.67E+0 5.58E-1 -1.41E+1
PENRM [MJ] 1.51E-1 0.00E+0 0.00E+0 0.00E+0 0.00E+0 0.00E+0 0.00E+0 0.00E+0
PENRT [MJ] 5.81E+1 1.98E+0 4.58E-1 0.00E+0 4.31E-2 1.67E+0 5.58E-1 -1.41E+1
SM [kg] 2.26E+0 0.00E+0 3.10E-2 0.00E+0 0.00E+0 0.00E+0 0.00E+0 0.00E+0
RSF [MJ] 5.13E+0 0.00E+0 0.00E+0 0.00E+0 0.00E+0 0.00E+0 0.00E+0 0.00E+0
NRSF [MJ] 5.73E+0 0.00E+0 0.00E+0 0.00E+0 0.00E+0 0.00E+0 0.00E+0 0.00E+0
FW [m³] 5.55E-1 3.36E-4 1.30E-4 0.00E+0 1.19E-5 2.83E-4 2.35E-4 -1.53E-3
PERE = Use of renewable primary energy excluding renewable primary energy resources used as raw materials; PERM = Use of
renewable primary energy resources used as raw materials; PERT = Total use of renewable primary energy resources; PENRE = Use of
non-renewable primary energy excluding non-renewable primary energy resources used as raw materials; PENRM = Use of non-
Caption
renewable primary energy resources used as raw materials; PENRT = Total use of non-renewable primary energy resources; SM = Use
of secondary material; RSF = Use of renewable secondary fuels; NRSF = Use of non-renewable secondary fuels; FW = Use of net fresh
water
RESULTS OF THE LCA – WASTE CATEGORIES AND OUTPUT FLOWS according to EN 15804+A1:
1 m2 A2 Natural Grey FUTURECEM, 25 mm, painted finish, delivered and used in Denmark
Parameter Unit A1-A3 A4 A5 B1 C1 C2 C4 D
HWD [kg] 6.47E-2 1.99E-3 1.51E-3 0.00E+0 5.40E-5 1.68E-3 1.24E-3 -4.88E-2
NHWD [kg] 1.97E+0 1.37E-1 1.15E-1 0.00E+0 1.12E-3 1.16E-1 5.18E-2 -1.66E+0
RWD [kg] 1.14E-4 1.35E-5 2.54E-6 0.00E+0 5.78E-7 1.14E-5 4.16E-6 -2.02E-5
CRU [kg] 6.83E-6 0.00E+0 0.00E+0 0.00E+0 0.00E+0 0.00E+0 0.00E+0 0.00E+0
MFR [kg] 1.62E-2 0.00E+0 0.00E+0 0.00E+0 0.00E+0 0.00E+0 0.00E+0 0.00E+0
MER [kg] 8.99E-3 0.00E+0 0.00E+0 0.00E+0 0.00E+0 0.00E+0 0.00E+0 0.00E+0
EEE [MJ] 0.00E+0 0.00E+0 0.00E+0 0.00E+0 0.00E+0 0.00E+0 1.45E+0 0.00E+0
EET [MJ] 0.00E+0 0.00E+0 0.00E+0 0.00E+0 0.00E+0 0.00E+0 4.65E+0 0.00E+0
HWD = Hazardous waste disposed; NHWD = Non-hazardous waste disposed; RWD = Radioactive waste disposed; CRU = Components
Caption for re-use; MFR = Materials for recycling; MER = Materials for energy recovery; EEE = Exported electrical energy; EET = Exported
thermal energy
6. LCA: Interpretation
The estimated impact results are only relative caused by the acquisition and use of cement, wood,
statements that do not indicate the end points of the and paint in the foreground processes. Global
impact categories, exceeding threshold values, safety Warming Potential net emissions share is much larger
margins or risks. in C4 than in A1-A3 (see why in chart (2)), while other
impact categories in module D, in general, are avoided
Two charts are presented: (1) with the standard in the waste system owing to the incineration of end-of-
lifecycle impact categories displaying the share of life panels and substitution of natural gas and Danish
impacts across all lifecycle stages, and (2) displaying electricity mix. C4 also slightly follows emissions of
the total carbon balance of the Troldekt product's compounds associated to other impact categories. A
lifecycle system. relatively inefficient transportation of end-of-life panels
to waste incineration causes emissions in especially
Impacts from the A1-A3 modules are dominant in the Abiotic depletion of non-fossil resources, Depletion of
life cycle of the Troldtekt A2 Natural Grey stratospheric ozone, and Photochemical ozone
FUTURECEM painted panel products. This is primarily formation.
The embodied emissions associated to the raw sequestered in A1-A3 and some fossil CO taken up in
2
materials (primarily cement and paint) are the main A1-A3 and B1 is re-emitted in C4. CO emissions
2-eq
cause of impacts, especially in terms of net Global occuring in the remaining modules are negligible.
Warming Potential, with respectively 4.85 kg CO
2-eq
and 0.4 kg CO followed by minor impacts from The amount of wood stored in the product refers to a
2-eq
additives. In general, direct emissions from the negative contribution to Global Warming Potential,
Troldtekt production site are relatively small. Abiotic reducing the share of Global Warming Potential in A1-
depletion of fossil resources appears from the burden A3. This is due to the sequestration of biogenic carbon
of producing cement using fossil raw material such as of wood during tree growth. The sequestered carbon
limestone and to a large extent fossil fuels. In terms of does not contribute to global warming as long as it is
carbon balance, biogenic CO in A1-A3 offsets nearly stored in the biomass.
2
all the fossil CO emissions in A1-A3. All biogenic CO
2 2
8 Environmental Product Declaration Troldtekt A/S – Troldtekt 25mm A2 Natural Grey FUTURECEM - painted
Summary Global Warming and Eutrophication, by order of
Within the cradle to grave, the following aspects have importance. The treatment of wastewater from the
been identified as major contributors, mainly in the painting cabin also contributes significantly to potential
categories Global Warming Potential and Abiotic impacts in terms of Eutrophication.
depletion of fossil resources:
The clinker (cement) production is the most critical
 Emissions from the clinker production from process of the Troldtekt product system, but
material inaccuracies around the amount used will not
invalidate the present conclusions.
 Emissions from the clinker production from
fuel
Notably, by introducing more up-to-date LCA datasets
 Substituted emissions from end of life for the grey cement applied, or introducing cements
incineration with less carbon footprint into production, as well as
improved paint consumption management, could lead
to significant reductions of especially the Global
Additionally, for painted panels, the manufacture of
Warming Potential indicator.
paint contribute significantly to impacts on potentials
for Photochemical ozone formation, Acidification,
7. Requisite evidence
Technological Institute under DANAK accreditation
7.1 Testing of substances used 392. Report no. MAIC-2019-1418. Reporting of
A detailed assessment of substances used was measured concentrations in toluene equivalents
conducted by a DAkkS-accredited laboratory, based according to EN 16516. This test is the basis for the
on a sample (prepared according to EN 15443), Finish M1 Material certificate as well as the Danish
available in the Test Report 2018P216294, using Indoor Climate labelling certificate.
inductively coupled plasma mass spectrometry (EN
16171) and X-ray fluorescence (EN 15309), for the AgBB overview of results (28 days [µg/m³])
following: Name Value Unit
 Heavy metals (cadmium, mercury, etc.) TVOC (C6 - C16) 12 μg/m3
 and other elements Sum SVOC (C16 - C22) 0 - 5 μg/m3
VOC without NIK 0 - 5 μg/m3
Carcinogenic Substances 1 μg/m3
7.2 Leaching
No leaching measurement was conducted according to
AgBB overview of results (3 days [µg/m³])
EN 717-1.
Name Value Unit
TVOC (C6 - C16) - μg/m3
Sum SVOC (C16 - C22) - μg/m3
7.3 VOC emissions
R (dimensionless) - -
Testing for VOC emissions has been conducted in
VOC without NIK - μg/m3
accordance with EN ISO 16000-6. Analysis of the air
Carcinogenic Substances - μg/m3
sampled on Tenax was performed at the Danish
8. References
Standards DIN 52612-2, Testing of thermal insulating materials;
determination of thermal conductivity by means of the
guarded hot plate apparatus; conversion of the
AgBB measured values for building applications. 1 June 1984
AgBB, Ausschuss zur gesundheitlichen Bewertung von
Bauprodukten (Committee for Health-related DIN EN ISO 14025
Evaluation of Building Products) DIN EN ISO 14025:2011, Environmental labels and
declarations – Type III environmental
BBSR declarations – Principles and procedures, German and
BBSR, Bundesinstitut für Bau-, Stadt- und English versions EN ISO 14025:2011
Raumforschung (Federal Institute for Research on
Building, Urban Affairs and Spatial Development). EN 13168
BBSR table: EN 13168:2012+A1:2015, Thermal insulation products
https://www.nachhaltigesbauen.de/fileadmin/pdf/baust for buildings. Factory made wood wool (WW) products.
off_gebauededaten/BNB_Nutzungsdauern_von_Bautei Specification
len_2017-02-24.pdf
EN 13964
DIN 4108-4 EN 13964:2014, Suspended ceilings. Requirements
DIN 4108-4:2017-03, Thermal insulation and energy and test methods
economy in buildings - Part 4: Hygrothermal design
values EN 15309
EN 15309:2007, Characterization of waste and soil.
DIN 52612-2
9 Environmental Product Declaration Troldtekt A/S – Troldtekt 25mm A2 Natural Grey FUTURECEM - painted
Determination of elemental composition by X-ray ISO 16000-6:2011, Indoor air - Part 6: Determination of
fluorescence volatile organic compounds in indoor and test chamber
air by active sampling on Tenax TA sorbent, thermal
EN 15443 desorption and gas chromatography using MS or MS-
EN 15443:2011, Solid recovered fuels. Methods for the FID
preparation of the laboratory sample
Product Category Rule A
EN 15804 Product Category Rule A, IBU, 2019, Part A,
EN 15804:2012, EN 15804:2012+A1 2013, Calculation Rules for the Life Cycle Assessment and
Sustainability of construction works – Environmental Requirements on the Project Report. v.1.8. IBU, 2019.
Product Declarations – Core rules for the product
category of construction products. Product Category Rule B
Product Category Rule B, IBU, 2019, Part B,
EN 16171 Requirements on the EPD for Wood cement - Mineral-
EN 16171:2016, Sludge, treated biowaste and soil. bonded wooden composites. v.1.7. IBU, 2019.
Determination of elements using inductively coupled
plasma mass spectrometry (ICP-MS) Regulation (EU) No. 305/2011
EN 16449
EN 16449:2014, EN 16449:2014, Wood and wood- Further References
based products - Calculation of the biogenic carbon
content of wood and conversion to carbon dioxide General Programme Instructions, IBU 2021
General Instructions for the EPD programme of Institut
EN 16516 Bauen und Umwelt e.V. Version 2.0, Berlin: Institut
EN 16516:2017+A1:2020, Construction products: Bauen und Umwelt e.V., 2021. www.ibu-epd.com
Assessment of release of dangerous substances.
Determination of emissions into indoor air Software/database
OneClick LCA software, Pre-verified EPD tool,
EN 717-1 Bionova: https://www.oneclicklca.com/
EN 717-1:2004, Wood-based Panels – Determination
of Formaldehyde Release – Formaldehyde emission Database: Ecoinvent v.3.6. cut-off (2019)
by the chamber method https://ecoinvent.org/the-ecoinvent-database/
European Waste Code: 10 13 11
(wastes from cement-based composite materials)
ISO 16000-6
10 Environmental Product Declaration Troldtekt A/S – Troldtekt 25mm A2 Natural Grey FUTURECEM - painted
Publisher
Institut Bauen und Umwelt e.V. Tel +49 (0)30 3087748- 0
Panoramastr. 1 Fax +49 (0)30 3087748- 29
10178 Berlin Mail info@ibu-epd.com
Germany Web www.ibu-epd.com
Programme holder
Institut Bauen und Umwelt e.V. Tel +49 (0)30 - 3087748- 0
Panoramastr 1 Fax +49 (0)30 – 3087748 - 29
10178 Berlin Mail info@ibu-epd.com
Germany Web www.ibu-epd.com
Author of the Life Cycle
Assessment Tel 98777223
Aalborg Portland Fax 80815733
Rørdalsvej 44 Mail
92200 Aalborg Ø stefan.e.danielsson@cementirhol
Denmark ding.it
Web www.aalborgportland.dk
Owner of the Declaration
Troldtekt A/S Tel +45 8747 8100
Sletvej 2A Fax +45 8747 8111
8310 Tranbjerg J Mail sales@troldtekt.dk
Denmark Web https://www.troldtekt.com
