ENVIRONMENTAL PRODUCT DECLARATION
as per ISO 14025 and EN 15804+A1
Owner of the Declaration Troldtekt A/S
Programme holder Institut Bauen und Umwelt e.V. (IBU)
Publisher Institut Bauen und Umwelt e.V. (IBU)
Declaration number EPD-TRO-20210110-ICA1-EN
Issue date 27.04.2021
Valid to 26.04.2026
Acoustic panels - unpainted
Troldtekt 25 mm Natural Grey
www.ibu-epd.com | https://epd-online.com
Umwelt Produktdeklaration Name des Herstellers – Name des Produkts
1. General Information
Troldtekt A/S Natural Grey, unpainted
Programme holder Owner of the declaration
IBU – Institut Bauen und Umwelt e.V. Troldtekt A/S
Panoramastr. 1 Sletvej 2 A
10178 Berlin 8310 Tranbjerg
Germany Denmark
Declaration number Declared product / declared unit
EPD-TRO-20210110-ICA1-EN Acoustic panel "Natural Grey" - 1m2, 25 mm thickness
- unpainted
This declaration is based on the product Scope:
category rules: This declaration represents the production, supply,
Wood cement - Mineral-bonded wooden composites, mounting, use, dismantling and disposal of 1 m2 (25
01.2019 mm thickness) of grey cement-bonded wood wool
(PCR checked and approved by the SVR) acoustic panel "Natural Grey", produced by Troldtekt
A/S, with a reference service life of 50 years. The
production facility is located in Jutland, Denmark.
Issue date
Three scenarios represent its use in indoor conditions
27.04.2021
in Denmark, Sweden and Germany.
Valid to
The owner of the declaration shall be liable for the
26.04.2026
underlying information and evidence; the IBU shall not
be liable with respect to manufacturer information, life
cycle assessment data and evidences.
The EPD was created according to the specifications
of EN 15804+A1. In the following, the standard will be
simplified as EN 15804.
Verification
The standard EN 15804 serves as the core PCR
Independent verification of the declaration and data
according to ISO 14025:2010
Dipl. Ing. Hans Peters internally x externally
(chairman of Institut Bauen und Umwelt e.V.)
Dr. Alexander Röder Ms Jane Anderson
(Managing Director Institut Bauen und Umwelt e.V.)) (Independent verifier)
2. Product
2.1 Product description/Product definition 2.2 Application
Troldtekt Natural Grey acoustic panels are some of the The panels are installed on the ceilings and walls in
leading and preferred solutions for creating a good offices,
indoor sound environment. They are sold in various businesses, schools, institutions, cultural sites, sports
thicknesses (20-35 mm) and dimensions (width: 600 centers, swimming pools and private homes.
mm, lengths: 600/1200/2400 mm or width: 625 mm,
lengths: 625/1250/2500 mm ). The panels can be 2.3 Technical Data
unpainted or painted in a wide variety of colors. The table below indicates the technical specifications
of the panels in accordance with EN 13168, the
For the placing on the market of the product in the standard for cement-bonded wood wool and double-
European Union/European Free Trade Association layer panels with cement-bonded wood wool, and EN
(EU/EFTA) (with the exception of Switzerland) 13964, the standard for suspended ceilings.
Regulation (EU) No. 305/2011 (CPR) applies. The
product needs a declaration of performance taking into
consideration EN 13964:2014, Suspended ceilings.
Requirements and test methods, and the CE-marking.
For the application and use, the respective national
provisions apply.
2 Environmental Product Declaration Troldtekt A/S – Troldtekt 25mm Natural Grey - unpainted
Technical specifications of the product covered in 2.9 Packaging
this EPD The product is packaged with plastic film and
Name Value Unit cardboard. The packaging material can be easily
Gross density 463 kg/m3 sorted and treated in dedicated waste recycling
Grammage 11,59 kg/m2 channels. The packaged product is delivered on a
Thermal conductivity acc. to DIN returnable wood pallet.
76 W/(mK)
52612
Water vapour diffusion resistance
- -
factor acc. to DIN 4108-4 2.10 Condition of use
Sound absorption coefficient (only with Conditions of use are detailed
reference to the corresponding - % here: https://www.troldtekt.com/Installation/Use_and_
component design) maintenance
Light reflection (measured by DELTA 26,3 -
Light and Optics 70,8 % 2.11 Environment and health during use
Reaction to fire B/S1/d0 Environmental and ecotoxicity risks from exposure to
Troldtekt panel products during use have been
assessed and found eligible to the following
certification schemes:
Performance data of the product in accordance with
the declaration of performance with respect to its  Finnish M1 classification
essential characteristics according to EN  Danish Indoor Climate
13168:2012+A1:2015, Thermal insulation products for
buildings. Factory made wood wool (WW) products.
These certificates can be accessed
Specification, and EN 13964:2014, Suspended
here: https://www.troldtekt.com/Web-
ceilings. Requirements and test methods.
tools/Downloads/Certificates-and-tests
2.4 Delivery status
2.12 Reference service life
The panel is usually distributed in length of 600, 1200
The technical service life of the panel is superior to 50
or 2400 mm by 600 mm width or in length of 625, 1250
years. This EPD refers to the service lifetime indicated
or 2500 mm by 625 mm width. It comes in three
by the BBSR table for the material 353.311 of type
thicknesses: 20, 25 and 35 mm. Additionally, several
“Holzbekleidungen: Holz, Holzwerkstoff und
density ranges are available: Coarse, Fine, Ultra-Fine
Mehrschichtleichtbauplatten”.
and Extreme-Fine causing different densities (388-428
kg/m3). The panels are normally delivered in packs of
Because the panel is used in a building, in this EPD its
80 units on pallets.
reference service life is limited by the expected service
life of the building, which is commonly accepted as 50
2.5 Base materials/Ancillary materials
years, at least as LCA timeframe.
The composition of the finished product is a mix of
wood wool (31,9%), Portland cement (62,2%), water
There is no influence of the ageing of the material on
(4,5%), as well as water glass (<1%) and accelerator
its technical performances.
(<1%). The composition is at dry basis at the factory
gate, as most of the water has evaporated during
2.13 Extraordinary effects
drying, but water remains bound to the wood fibre and
cement paste (hydrated cement).
Fire
Information on the fire performance according to EN
2.6 Manufacture
13168.
Norway spruce logs from local forests (with a moisture
content of about 65-70%) are received and the bark is
Fire protection
removed. The wood is stored for approximately six
Name Value
months until the moisture content in the wood drops to
Building material class B
29%. The wood is then shredded to produce wool. The
Burning droplets d0
wood wool is mixed together with Portland cement,
Smoke gas development S1
water, and additives. The mixture is cast and cured
using a heat press and dried with a biomass-fired
Water
oven. The cast panel is milled to remove any material
No information on the product performance under the
in excess and cut edges. After approximately 4 weeks
unforseeable influence of water is available.
of curing, the panel can be painted before being stored
on a pallet and packaged to be transported to central
Mechanical destruction
distribution warehouses.
No information on the product performance under
unforseeable mechanical destruction is available.
2.7 Environment and health during
manufacturing
2.14 Re-use phase
Troldtekt is following its working environment closely.
Currently, Troldtekt panels undergo thermal treatment
Both the physical working environment and sickness
with energy recovery. Composting is also possible.
absence are closely monitored. It is an ongoing
process involving both leaders and factory workers.
Additional information on recycling
options: https://www.troldtekt.com/~/media/Files/Info%
2.8 Product processing/Installation
20sheets/English/Troldtekt_Recycling%20instructions
Installation instructions are available here:
%20pdf.pdf
https://www.troldtekt.com/Installation
3 Environmental Product Declaration Troldtekt A/S – Troldtekt 25mm Natural Grey - unpainted
2.15 Disposal Additional information on disposal
The product may be composted, thermally treated with options: https://www.troldtekt.com/environment-and-
energy recovery, or landfilled. csr/product-life-cycle/recycling/
European Waste Code: 10 13 11 (wastes from 2.16 Further information
cement-based composite materials) For additional information on technical specifications,
you may consult the Declaration Of
Painted panels must be incinerated at end-of-life. Performance: https://www.troldtekt.com/Web-
tools/Downloads/DoPs
3. LCA: Calculation rules
3.1 Declared Unit entirety of the annual production of panels in 2020 and
The functional unit is 1 m2 of acoustic panel, in 25 mm is verified by a third party. Such representativeness is
thickness, corresponding to 11,59 kg of material with also valid for the production of Portland cement, whose
unpainted finish, mounted on ceiling, with a reference EPDs, however, were published in 2021 (white) and
service life of 50 years. 2017 (grey).
Declared unit Temporal, geographical and technological
Name Value Unit representativeness
Declared unit 1 m2 All data strictly related to the cement production is
Gross density 463 kg/m3 technologically, temporally, and geographically
Grammage 11.59 kg/m2 representative. The cement production data is less
conversion factor [Mass/Declared than 5 years old. However, since the improvement in
11.59 -
Unit] grey cement production processes in the meantime
Layer thickness 0.025 m have not been accounted for, the LCA results for the
Troldtekt panels based on grey cement can be said to
be conservative. The data used to model the
foreground inventory of acoustic panels dates from the
3.2 System boundary production year of 2020. As for secondary data, some
Cradle to grave most of the ecoinvent datasets are less than 3 years
old.
3.3 Estimates and assumptions
Assumptions are described occasionally throughout 3.7 Period under review
the section "LCA: Calculation rules". The primary data concerned with the manufacture (A1-
A3) relates to the production year 2020 and the data
3.4 Cut-off criteria are based on the volumes produced on an annual
The cut-off criterion is applied according to EN basis.
15804 Section 6.3.5 and PCR part A Section 5.6.
All inputs and outputs for which data are available are 3.8 Allocation
included in the LCA model. Data gaps are filled with Allocation of production data to the multiple produced
conservative assumptions from average data (when types of panels (with the same functional unit) is
available) or with generic data and are documented performed based on the rules provided in EN 15804.
accordingly. Sub-processes associated to painting have specially
The following product flows have been omitted been allocated to the painted panels. Data such as
according to the 1% cut-off rule: waste generation and packaging have been allocated
 Wooden pallet to transport the product to the entire production volume of panels in Troldtekt.
The only case of co-produced outputs is associated to
 Capital infrastructure (factory)
wood logging. However, the environmental load is
 Allocation of burden from wood logging to
evenly distributed over all its co-products, such as
residual wood fractions logs, energy wood, and bark.
3.9 Comparability
Basically, a comparison or an evaluation of EPD data
3.5 Background data
is only possible if all the data sets to be compared
Two types of data source are used as secondary data:
were created according to EN 15804 and the building
 Product-specific EPDs for the manufacture
context, respectively the product-specific
and supply of Portland cement and water-
characteristics of performance, are taken into account.
based paint
 Database ecoinvent v.3.6 cut-off The used background database is ecoinvent v.3.6 cut-
off
3.6 Data quality
Statistical representativeness
The statistical representativeness of the product
system is very good. The input and output data
samples used to build inventories are based on the
4. LCA: Scenarios and additional technical information
4 Environmental Product Declaration Troldtekt A/S – Troldtekt 25mm Natural Grey - unpainted
Manufacture (A1-A3) Name Value Unit
Electricity consumption 0,060 kWh
Data Material loss (plastic film) 0,007 kg
Primary data is third-party verified and based on the Material loss (cardborad) 0,032 kg
production year 2020, within the facilities of Troldtekt
A/S in Jutland (Denmark). Use phase (B1)
Prior to distribution and during the use phase (B1), the
End-of-waste state and use of by-products carbonation of the cement contained in the panel,
For all processes supplying a residual material/waste during use, is accounted for. Based on laboratory
that originates the end-of-life phase of a product to the measurement, the panel will absorb up to 140 grams of
product system to be used as input, the polluter-pay carbon dioxide per kilogram of cement. Normalized to
principle “100:0” is used. Some wooden by-products the reference flow, this corresponds to an uptake of
generated during manufacture in Troldtekt end up as approximately 0,9 kilograms of carbon dioxide by the
soil improvers externally (reaching end-of-waste state), end of the service lifetime, including the uptake in A3.
and thus their biogenic carbon leaves Troldtekt's
system boundary. Information about reference service life is detailed in
2.12.
Wind-certified electricity
All the electricity used to produce the panels in the Reference service life
Module A3 originates from Danish wind power, for Name Value Unit
which a certificate ensures the origin. It originates from Reference service life (according to
50 a
a 1-3 MW offshore wind turbine, with transformation, ISO 15686-1, -2, -7 and -8)
transmission and distribution losses and is modelled Life Span (according to BBSR) 50 a
correspondingly. Life Span according to the
manufacturer
75 a
Carbon balance
Biogenic: Absorption of biogenic CO2 by the End of life (C1-C4)
purchased wood has been considered in A1. Some of
Name Value Unit
it is released again during production in A3, some ends Electricity use (for un-mounting) 0,060 kWh
up sequestered in soil, while the majority of the
Transport (to material sorting facility) 50 km
remaining biogenic CO2, 7,15 kg, is retained in the
Collected as mixed construction waste 11,59 kg
finished product and emitted during end-of-life
Energy recovery 3,64 kg
incineration in C4.
Energy recovery efficiency 10 %
Fossil: Absorption of some fossil CO2, originating from
Energy recovered 7,42 MJ
the calcination of limestone during cement production,
happens when the cement is mixed with water in A3. A
The panel is un-mounted at the end of its reference
majority is absorbed during the use phase B1, and all
service life and driven to the regional waste
the absorbed fossil CO2 is finally emitted during end-
incineration plant. Energy is recovered from the wood
of-life incineration in C4.
part of the panel at 10% efficiency.
Distribution to site (A4) and mounting (A5)
To consider the main geographical variants of the life
cycle of Troldtekt Natural Grey panels, three scenarios Reuse, recovery and/or recycling potentials (D),
are developed, where the product is supplied, relevant scenario information
mounted, used and discarded in Aarhus (Denmark), Name Value Unit
Hamburg (Germany) and Malmö (Sweden). An Electricity 1,76 MJ
additional 50 km from the local warehouse to Heat 5,66 MJ
construction site is assumed.
The energy substituted from incineration of the panel's
wood component in C4 is considered being a split of
Transport to the building site (A4) the Danish electricity grid mix (for electricity) and
Name Value Unit natural gas (for heat).
Litres of fuel 26,8 l/100km
Transport distance to Denmark 160 km Details on possible disposal routes
Transport distance to Germany 370 km Aalborg Portland cement factory utilizes dust and
Transport distance to Sweden 394 km offcuts from the Troldtekt factory as a raw material in
Transport distance from new cement, i.e. in the technical circle. During
warehouse to local construction incineration in the cement kiln, the wood content in the
50 km
sites in cement bonded wood wool panels replaces fossil fuels,
Denmark/Germany/Sweden while the cement ends up as a raw material in new
Capacity utilisation (including cement, replacing virgin raw materials and heavy fossil
empty runs) 85 % fuels, thereby avoiding a significant amount of CO 2
emissions. This scheme of wood wool waste as a raw
Gross density of products
463 kg/m3 material can be scaled for construction site and
transported
demolition waste. It will be gradually rolled out to all of
Capacity utilisation volume factor 1 -
Denmark in the period 2021-2023. Once Denmark has
documented economic and environmental benefits to
be gained by including wood wool waste in the
production of new cement rather than going to waste
incineration or landfill, dialogue with municipalities and
Installation into the building (A5)
local cement producers in the primary markets of
5 Environmental Product Declaration Troldtekt A/S – Troldtekt 25mm Natural Grey - unpainted
Troldtekt is initiated to facilitate similar schemes
regionally or nationally.
6 Environmental Product Declaration Troldtekt A/S – Troldtekt 25mm Natural Grey - unpainted
5. LCA: Results
Note: Global Warming Potential (GWP) indicator includes CO2 of both biogenic and fossil origin.
Also, GWP results for Troldtekt Natural Grey (unpainted) for other delivery scenarios in respectively Germany and
Sweden, are 2,27E-1 kg CO2 and 2,40E-1 kg CO2.
DESCRIPTION OF THE SYSTEM BOUNDARY (X = INCLUDED IN LCA; MND = MODULE NOT DECLARED;
MNR = MODULE NOT RELEVANT)
BENEFITS AND
CONSTRUCTI LOADS
PRODUCT STAGE ON PROCESS USE STAGE END OF LIFE STAGE BEYOND THE
STAGE SYSTEM
BOUNDARIES
7 Environmental Product Declaration Troldtekt A/S – Troldtekt 25mm Natural Grey - unpainted
lairetam
waR
ylppus tropsnarT
gnirutcafunaM
eht
morf
tropsnarT
etis
eht
ot
etag
ylbmessA esU
ecnanetniaM
riapeR
tnemecalpeR tnemhsibrufeR
ygrene
lanoitarepO esu
retaw
lanoitarepO esu
noitcurtsnoc-eD
noitilomed tropsnarT
gnissecorp
etsaW
lasopsiD -esueR -yrevoceR -gnilcyceR laitnetop
A1 A2 A3 A4 A5 B1 B2 B3 B4 B5 B6 B7 C1 C2 C3 C4 D
X X X X X X MND MNR MNR MNR MND MND X X MND X X
RESULTS OF THE LCA - ENVIRONMENTAL IMPACT according to EN 15804+A1: 1 m2 Natural Grey, 25
mm, unpainted, delivered and used in Denmark
Parameter Unit A1-A3 A4 A5 B1 C1 C2 C4 D
GWP [kg CO2-Eq.] 6.77E-1 1.14E-1 8.76E-2 -7.80E-1 6.50E-4 9.59E-2 8.18E+0 -9.69E-1
ODP [kg CFC11-Eq.] 2.40E-7 2.08E-8 1.64E-9 0.00E+0 2.81E-10 1.75E-8 6.52E-9 -5.36E-8
AP [kg SO2-Eq.] 1.47E-2 2.30E-4 5.90E-5 0.00E+0 1.59E-6 1.94E-4 5.38E-4 -2.01E-3
EP [kg (PO4)3--Eq.] 6.04E-3 4.73E-5 1.03E-4 0.00E+0 8.86E-7 3.98E-5 2.34E-4 -1.49E-3
POCP [kg ethene-Eq.] 7.30E-4 1.52E-5 2.58E-6 0.00E+0 8.88E-8 1.28E-5 4.22E-5 -1.16E-4
ADPE [kg Sb-Eq.] 3.27E-5 3.11E-6 2.09E-7 0.00E+0 1.82E-8 2.61E-6 7.10E-7 -2.60E-6
ADPF [MJ] 4.50E+1 1.71E+0 2.93E-1 0.00E+0 4.76E-3 1.44E+0 5.18E-1 -1.57E+1
GWP = Global warming potential; ODP = Depletion potential of the stratospheric ozone layer; AP = Acidification potential of land and water; EP =
Caption Eutrophication potential; POCP = Formation potential of tropospheric ozone photochemical oxidants; ADPE = Abiotic depletion potential for non-
fossil resources; ADPF = Abiotic depletion potential for fossil resources
RESULTS OF THE LCA - INDICATORS TO DESCRIBE RESOURCE USE according to EN 15804+A1: 1 m2
Natural Grey, 25 mm, unpainted, delivered and used in Denmark
Parameter Unit A1-A3 A4 A5 B1 C1 C2 C4 D
PERE [MJ] 6.23E+1 2.44E-2 1.60E-1 0.00E+0 3.91E-2 2.06E-2 8.59E+0 -6.34E+0
PERM [MJ] 7.47E+1 0.00E+0 0.00E+0 0.00E+0 0.00E+0 0.00E+0 0.00E+0 0.00E+0
PERT [MJ] 1.37E+2 2.44E-2 1.60E-1 0.00E+0 3.91E-2 2.06E-2 8.59E+0 -6.34E+0
PENRE [MJ] 4.64E+1 1.74E+0 4.58E-1 0.00E+0 4.31E-2 1.47E+0 6.79E-1 -1.71E+1
PENRM [MJ] 0.00E+0 0.00E+0 0.00E+0 0.00E+0 0.00E+0 0.00E+0 0.00E+0 0.00E+0
PENRT [MJ] 4.64E+1 1.74E+0 4.58E-1 0.00E+0 4.31E-2 1.47E+0 6.79E-1 -1.71E+1
SM [kg] 2.26E+0 0.00E+0 3.10E-2 0.00E+0 0.00E+0 0.00E+0 0.00E+0 0.00E+0
RSF [MJ] 5.13E+0 0.00E+0 0.00E+0 0.00E+0 0.00E+0 0.00E+0 0.00E+0 0.00E+0
NRSF [MJ] 5.73E+0 0.00E+0 0.00E+0 0.00E+0 0.00E+0 0.00E+0 0.00E+0 0.00E+0
FW [m³] 3.40E-2 2.96E-4 1.30E-4 0.00E+0 1.19E-5 2.49E-4 2.86E-4 -1.86E-3
PERE = Use of renewable primary energy excluding renewable primary energy resources used as raw materials; PERM = Use of
renewable primary energy resources used as raw materials; PERT = Total use of renewable primary energy resources; PENRE = Use of
non-renewable primary energy excluding non-renewable primary energy resources used as raw materials; PENRM = Use of non-
Caption
renewable primary energy resources used as raw materials; PENRT = Total use of non-renewable primary energy resources; SM = Use
of secondary material; RSF = Use of renewable secondary fuels; NRSF = Use of non-renewable secondary fuels; FW = Use of net fresh
water
RESULTS OF THE LCA – WASTE CATEGORIES AND OUTPUT FLOWS according to EN 15804+A1:
1 m2 Natural Grey, 25 mm, unpainted, delivered and used in Denmark
Parameter Unit A1-A3 A4 A5 B1 C1 C2 C4 D
HWD [kg] 5.09E-2 1.76E-3 1.51E-3 0.00E+0 5.40E-5 0.00E+0 1.50E-3 -5.92E-2
NHWD [kg] 1.66E+0 1.21E-1 1.15E-1 0.00E+0 1.12E-3 0.00E+0 6.31E-2 -2.02E+0
RWD [kg] 7.82E-5 1.19E-5 2.54E-6 0.00E+0 5.78E-7 0.00E+0 5.06E-6 -2.45E-5
CRU [kg] 0.00E+0 0.00E+0 0.00E+0 0.00E+0 0.00E+0 0.00E+0 0.00E+0 0.00E+0
MFR [kg] 1.05E-2 0.00E+0 0.00E+0 0.00E+0 0.00E+0 0.00E+0 0.00E+0 0.00E+0
MER [kg] 4.86E-3 0.00E+0 0.00E+0 0.00E+0 0.00E+0 0.00E+0 0.00E+0 0.00E+0
EEE [MJ] 0.00E+0 0.00E+0 0.00E+0 0.00E+0 0.00E+0 0.00E+0 1.76E+0 0.00E+0
EET [MJ] 0.00E+0 0.00E+0 0.00E+0 0.00E+0 0.00E+0 0.00E+0 5.66E+0 0.00E+0
HWD = Hazardous waste disposed; NHWD = Non-hazardous waste disposed; RWD = Radioactive waste disposed; CRU = Components
Caption for re-use; MFR = Materials for recycling; MER = Materials for energy recovery; EEE = Exported electrical energy; EEE = Exported
thermal energy
6. LCA: Interpretation
The estimated impact results are only relative cement and wood in the foreground processes. Global
statements which do not indicate the end points of the Warming Potential net emissions share is much larger
impact categories, exceeding threshold values, safety in C4 than in A1-A3 (see why in chart (2)), while other
margins or risks. impact categories in module D in general are avoided
in the waste system owing to the incineration of end-of-
Two charts are presented: (1) with the standard life panels and substitution of natural gas and Danish
lifecycle impact categories displaying the share of electricity mix. C4 also slightly follows emissions of
impacts across all lifecycle stages, and (2) displaying compounds associated to other impact categories. A
the total carbon balance of the Troldekt product's relatively inefficient transportation of end-of-life panels
lifecycle system. to waste incineration causes emissions in especially
Abiotic depletion of non-fossil resources, Depletion of
Impacts from the A1-A3 modules are dominant in the stratospheric ozone, and Photochemical ozone
life cycle of the Troldtekt Natural Grey panel products. formation.
This is primarily caused by the acquisition and use of
The embodied emissions associated to the raw A1-A3 and some fossil CO2 taken up in A1-A3 and B1
materials (primarily cement) are the main cause of is re-emitted in C4. CO2-eq emissions ocuring in the
impacts, especially in terms of net Global Warming remaining modules are negligible.
Potential, with 7,2 kg CO2-eq for cement followed by
minor impacts from additives. In general, direct The amount of wood stored in the product refers to a
emissions from the Troldtekt production site are negative contribution to Global Warming Potential,
relatively small. Abiotic depletion of fossil resources reducing the share of Global Warming Potential in A1-
appears from the burden of producing cement using A3. This is due to the sequestration of biogenic carbon
fossil raw material such as limestone and to a large of wood during tree growth. The sequestered carbon
extent fossil fuels. In terms of carbon balance, biogenic does not contribute to global warming as long as it is
CO2 in A1-A3 offsets nearly all the fossil CO2 stored in the biomass.
emissions in A1-A3. All biogenic CO2 sequestered in
8 Environmental Product Declaration Troldtekt A/S – Troldtekt 25mm Natural Grey - unpainted
Summary
Within the cradle to grave, the following aspects have The clinker (cement) production is the most critical
been identified as major contributors, mainly in the process of the Troldtekt product system, but
categories Global Warming Potential and Abiotic inaccuracies around the amount used will not
depletion of fossil resources: invalidate the present conclusions.
 Emissions from the clinker production from Notably, by introducing more up-to-date LCA datasets
material for the grey cement applied, or introducing cements
with less carbon footprint into production could lead to
 Emissions from the clinker production from
significant reductions of especially the Global Warming
fuel
Potential indicator.
 Substituted emissions from end of life
incineration
7. Requisite evidence
7.3 VOC emissions
7.1 Testing of substances used Testing for VOC emissions has been conducted in
A detailed assessment of substances used was accordance with EN ISO 16000-6. Analysis of the air
conducted by a DAkkS-accredited laboratory, based sampled on Tenax was performed at the Danish
on a sample (prepared according to EN 15443), Technological Institute under DANAK accreditation
available in the Test Report 2018P216294, using 392. Report no. MAIC-2019-1418. Reporting of
inductively coupled plasma mass spectrometry (EN measured concentrations in toluene equivalents
16171) and X-ray fluorescence (EN 15309), for the according to EN 16516. This test is basis for the Finish
following: M1 Material certificate as well as the Danish Indoor
 Heavy metals (cadmium, mercury, etc.) Climate labeling certificate.
 and other elements
AgBB overview of results (28 days [µg/m³])
Name Value Unit
7.2 Leaching TVOC (C6 - C16) 12 μg/m3
No leaching measurement was conducted according Sum SVOC (C16 - C22) 0 - 5 μg/m3
to EN 717-1. VOC without NIK 0 - 5 μg/m3
Carcinogenic Substances 1 μg/m3
8. References
Standards declarations – Principles and procedures, German and
English versions EN ISO 14025:2011
AgBB
AgBB, Ausschuss zur gesundheitlichen Bewertung von EN 13168
Bauprodukten (Committee for Health-related EN 13168:2012+A1:2015, Thermal insulation products
Evaluation of Building Products) for buildings. Factory made wood wool (WW) products.
Specification
BBSR
BBSR, Bundesinstitut für Bau-, Stadt- und EN 13964
Raumforschung (Federal Institute for Research on EN 13964:2014, Suspended ceilings. Requirements
Building, Urban Affairs and Spatial Development). and test methods
BBSR table:
https://www.nachhaltigesbauen.de/fileadmin/pdf/baust EN 15309
off_gebauededaten/BNB_Nutzungsdauern_von_Bautei EN 15309:2007, Characterization of waste and soil.
len_2017-02-24.pdf Determination of elemental composition by X-ray
fluorescence
DIN 4108-4
DIN 4108-4:2017-03, Thermal insulation and energy EN 15443
economy in buildings - Part 4: Hygrothermal design EN 15443:2011, Solid recovered fuels. Methods for the
values preparation of the laboratory sample
DIN 52612-2 EN 15804
DIN 52612-2, Testing of thermal insulating materials; EN 15804:2012, EN 15804:2012+A1 2013,
determination of thermal conductivity by means of the Sustainability of construction works – Environmental
guarded hot plate apparatus; conversion of the Product Declarations – Core rules for the product
measured values for building applications. 1 June 1984 category of construction products.
DIN EN ISO 14025 EN 16171
DIN EN ISO 14025:2011, Environmental labels and EN 16171:2016, Sludge, treated biowaste and soil.
declarations – Type III environmental Determination of elements using inductively coupled
plasma mass spectrometry (ICP-MS)
9 Environmental Product Declaration Troldtekt A/S – Troldtekt 25mm Natural Grey - unpainted
EN 16449 Product Category Rule B
EN 16449:2014, EN 16449:2014, Wood and wood- Product Category Rule B, IBU, 2019, Part B,
based products - Calculation of the biogenic carbon Requirements on the EPD for Wood cement - Mineral-
content of wood and conversion to carbon dioxide bonded wooden composites. v.1.7. IBU, 2019.
EN 16516
EN 16516:2017+A1:2020, Construction products: Further References
Assessment of release of dangerous substances.
Determination of emissions into indoor air General Programme Instructions, IBU 2016
General Programme Instructions for the Preparation of
EN 717-1 EPDs at the Institut Bauen und Umwelt e.V. Version 1.,
EN 717-1:2004, Wood-based Panels – Determination Berlin: Institut Bauen und Umwelt e.V., 2016.
of Formaldehyde Release – Formaldehyde emission
by the chamber method Software/database
OneClick LCA software, Pre-verified EPD tool,
ISO 16000-6 Bionova: https://www.oneclicklca.com/
ISO 16000-6:2011, Indoor air - Part 6: Determination of
volatile organic compounds in indoor and test chamber Database: Ecoinvent v.3.6. cut-off (2019)
air by active sampling on Tenax TA sorbent, thermal
desorption and gas chromatography using MS or MS-
FID
Product Category Rule A
Product Category Rule A, IBU, 2019, Part A,
Calculation Rules for the Life Cycle Assessment and
Requirements on the Project Report. v.1.8. IBU, 2019.
10 Environmental Product Declaration Troldtekt A/S – Troldtekt 25mm Natural Grey - unpainted
Publisher
Institut Bauen und Umwelt e.V. Tel +49 (0)30 3087748- 0
Panoramastr. 1 Fax +49 (0)30 3087748- 29
10178 Berlin Mail info@ibu-epd.com
Germany Web www.ibu-epd.com
Programme holder
Institut Bauen und Umwelt e.V. Tel +49 (0)30 - 3087748- 0
Panoramastr 1 Fax +49 (0)30 – 3087748 - 29
10178 Berlin Mail info@ibu-epd.com
Germany Web www.ibu-epd.com
Author of the Life Cycle
Assessment Tel 98777223
Aalborg Portland Fax 80815733
Rørdalsvej 44 Mail
92200 Aalborg Ø stefan.e.danielsson@cementirhol
Denmark ding.it
Web www.aalborgportland.dk
Owner of the Declaration
Troldtekt A/S Tel +45 8747 8100
Sletvej 2A Fax +45 8747 8111
8310 Tranbjerg J Mail sales@troldtekt.dk
Denmark Web https://www.troldtekt.com
