ENVIRONMENTAL PRODUCT DECLARATION
as per ISO 14025 and EN 15804+A2
Owner of the Declaration dormakaba International Holding GmbH
Publisher Institut Bauen und Umwelt e.V. (IBU)
Programme holder Institut Bauen und Umwelt e.V. (IBU)
Declaration number EPD-DOR-20220164-CBA1-EN
Issue date 19.10.2022
Valid to 18.10.2027
TS 71/TS 72
dormakaba
www.ibu-epd.com | https://epd-online.com
General Information
dormakaba TS 71/TS 72
Programme holder Owner of the declaration
IBU – Institut Bauen und Umwelt e.V. dormakaba International Holding GmbH
Hegelplatz 1 DORMA Platz 1
10117 Berlin 58256 Ennepetal
Germany Germany
Declaration number Declared product / declared unit
EPD-DOR-20220164-CBA1-EN 1 door closer (1 piece) TS 71/TS 72
This declaration is based on the product category rules: Scope:
Building Hardware products, 01.08.2021 This Environment Product Declaration refers to a specific door closer
(PCR checked and approved by the SVR) manufactured by dormakaba China Ltd. The production site is located in
Suzhou (China).
Issue date The data represents the year 2020.
The owner of the declaration shall be liable for the underlying information
19.10.2022
and evidence; the IBU shall not be liable with respect to manufacturer
information, life cycle assessment data and evidences.
Valid to
The EPD was created according to the specifications of EN 15804+A2. In
18.10.2027 the following, the standard will be simplified as EN 15804.
Verification
The standard EN 15804 serves as the core PCR
Independent verification of the declaration and data according to ISO
14025:2011
internally X externally
Dipl.-Ing. Hans Peters
(Chairman of Institut Bauen und Umwelt e.V.)
Florian Pronold Dr.-Ing. Wolfram Trinius,
(Managing Director Institut Bauen und Umwelt e.V.) (Independent verifier)
1 Environmental Product Declaration - dormakaba - TS 71/TS 72
Product
Product description/Product definition
The TS 71/TS 72 are the ideal multi-purpose door closers for all
standard door designs and constructions. Without a backplate,
it is particularly easy and quick to fix. The spring strength can
be individually adapted to the door size by means of an
adjusting valve. For the use and application of the product the
respective national provisions at the place of use apply. The
standards which can be applied are the following:
• EN 1154
• EN 1634-1
Application
The door closers can be used for all standard doors (single-
and double-leaf doors).
Technical Data
The door closer has following technical properties:
Performance data of the product with respect to its
characteristics in accordance with the relevant technical
provision which can be applied are mentioned above.
Base materials/Ancillary materials
The major material compositions including the packaging of the
product are listed below:
Name Value Unit
Steel 64 %
Aluminium 20 %
Paper 7 %
Plastics 4 %
Lubricants 4 %
Zinc 1 %
The product includes partial articles which contain substances
listed in the Candidate List of REACH Regulation
1907/2006/EC (date: 17.01.2022) exceeding 0.1 percentage by
mass: yes
• Lead (Pb): 7439-92-1 (CAS-No.) is included in some of
the alloys used. The concentration of lead in each
individual alloy does not exceed 4.0% (by mass).
The Candidate List can be found on the ECHA website
address: https:echa.europa.eu/de/home.
Reference service life
The reference service life of the TS 71/TS 72 door closers
depend on the traffic pattern and degree of usage of the door.
These closers are rated to EN 1154, meaning they are
designed to withstand a minimum of 500,000 cycles. The
reference service life amounts for 20 years. This corresponds
with approx. 25,000 cycles per year.
2 Environmental Product Declaration - dormakaba - TS 71/TS 72
LCA: Calculation rules
final residues during the construction process stage.
Declared Unit
The declared unit is 1 piece of the product: TS 71/TS 72. End-of-life stage– Modules C1-C4 and D
Declared unit The end-of-life stage includes:
— C1, de-construction, demolition:
Name Value Unit
— C2, transport to waste processing;
Declared unit 1 piece/product
— C3, waste processing for reuse, recovery and/or recycling;
Mass of declared Product 1.74 kg — C4, disposal;
including provision and all transport, provision of all materials,
System boundary products and related energy and water use.
The type of EPD is: cradle to gate with options, modules C1–
C4, and module D (A1–A3 + C + D and additional modules: A4
+ A5) Module D (Benefits and loads beyond the system boundary)
includes:
Production - Module A1-A3 — D, recycling potentials, expressed as net impacts and
The product stage includes: benefits.
— A1, raw material extraction, processing and mechanical
Geographic Representativeness
treatments, processing of secondary material input (e.g.
Land or region, in which the declared product system is
recycling processes), — A2, transport to the manufacturer,
manufactured, used or handled at the end of the product´s
— A3, manufacturing and assembly including provision of all
lifespan: China
materials, products and energy, as well as waste processing up
to the end-of waste state.
Comparability
Construction stage - Modules A4-A5
Basically, a comparison or an evaluation of EPD data is only
The construction process stage includes:
possible if all the data sets to be compared were created
— A4, transport to the building site;
according to EN 15804 and the building context, respectively
— A5, installation into the building;
the product-specific characteristics of performance, are taken
including provision of all materials, products and energy, as well
into account.
as waste processing up to the end-of waste state or disposal of
LCA: Scenarios and additional technical information
Installation into the building (A5)
Characteristic product properties of biogenic carbon
Name ValueUnit
Information on describing the biogenic Carbon Content at
Output substances following waste treatment on
factory gate 0.09 kg
site (paper packaging)
Name ValueUnit
kg End of life (C1-C4)
Biogenic carbon content in product 0.01
C C1: The product dismantling from the building is done manually
Biogenic carbon content in accompanying kg without environmental burden.
0.03
packaging C C2: Transport to waste treatment at end of life is 50km.
Note: 1 kg of biogenic carbon is equivalent to 44/12 kg of CO . Name Value Unit
2
Collected separately waste type 2.47 kg
Recycling 2.46 kg
Additional technical information for the declared modules. Energy recovery 0.01 kg
Transport to the building site (A4)
Reuse, recovery and/or recycling potentials (D), relevant
Name Value Unit
scenario information
Litres of fuel truck (per piece) 0.00276l/100km
Name Value Unit
Transport distance (truck) 500 km
Recycling 100 %
Capacity utilisation (including empty runs)
55 % Collection rate is 100%.
average
Transport distance (ship) 10000 km
3 Environmental Product Declaration - dormakaba - TS 71/TS 72
LCA: Results
DESCRIPTION OF THE SYSTEM BOUNDARY (X = INCLUDED IN LCA; MND = MODULE OR INDICATOR NOT DECLARED; MNR
= MODULE NOT RELEVANT)
Benefits and
Construction loads beyond
Product stage Use stage End of life stage
process stage the system
boundaries
la ire ta m w a Ry lp p u s tro p s n a rT g n iru tc a fu n a M e h t m o rf tro p s n a rTe tis e h t o t e ta g y lb m e s s A e s U e c n a n e tn ia M ria p e R tn e m e c a lp e R tn e m h s ib ru fe R y g re n e la n o ita re p Oe s u re ta w la n o ita re p Oe s u n o itc u rts n o c -e Dn o itilo m e d tro p s n a rT g n is s e c o rp e ts a W la s o p s iD -e s u e R-y re v o c e R-g n ilc y c e Rla itn e to p
A1 A2 A3 A4 A5 B1 B2 B3 B4 B5 B6 B7 C1 C2 C3 C4 D
X X X X X MND MND MNR MNR MNR MND MND X X X X X
RESULTS OF THE LCA - ENVIRONMENTAL IMPACT according to EN 15804+A2: 1 door closer
Parameter Unit A1-A3 A4 A5 C1 C2 C3 C4 D
GWP-total kg CO 2 eq 1.3E+01 1.33E-01 1.57E-01 0 7E-03 4.15E-01 0 -2.9E+00
GWP-fossil kg CO 2 eq 1.32E+01 1.3E-01 4E-03 0 7E-03 3.92E-01 0 -2.89E+00
GWP-biogenic kg CO 2 eq -1.86E-01 3E-03 1.53E-01 0 3.15E-04 2.3E-02 0 -7E-03
GWP-luluc kg CO 2 eq 7.01E-03 2.9E-06 2.59E-06 0 1.62E-07 2.24E-05 0 -5.79E-04
ODP kg CFC11 eq 2.11E-10 1.31E-17 2.84E-17 0 7.19E-19 2.01E-16 0 -1.81E-11
AP mol H+ eq 6.26E-02 2E-03 4.41E-05 0 6.81E-06 7.31E-05 0 -1.1E-02
EP-freshwater kg P eq 9.91E-06 2.84E-08 5.55E-09 0 1.46E-09 3.19E-08 0 -1.58E-06
EP-marine kg N eq 1.02E-02 5.76E-04 1.59E-05 0 2.17E-06 1.68E-05 0 -1E-03
EP-terrestrial mol N eq 1.1E-01 6E-03 1.98E-04 0 2.41E-05 3.33E-04 0 -1.6E-02
kg NMVOC
POCP 3.15E-02 2E-03 4.22E-05 0 6.13E-06 4.65E-05 0 -5E-03
eq
ADPE kg Sb eq 1.76E-04 3.64E-09 4.48E-10 0 2.04E-10 2.76E-09 0 -4.44E-05
ADPF MJ 1.38E+02 1.72E+00 5E-02 0 9.7E-02 1.87E-01 0 -3.93E+01
m3 world eq
WDP 2.48E+00 2.45E-04 2E-02 0 1.33E-05 4.2E-02 0 -1.39E-01
deprived
GWP = Global warming potential; ODP = Depletion potential of the stratospheric ozone layer; AP = Acidification potential of land and water; EP =
Eutrophication potential; POCP = Formation potential of tropospheric ozone photochemical oxidants; ADPE = Abiotic depletion potential for non-fossil
resources; ADPF = Abiotic depletion potential for fossil resources; WDP = Water (user) deprivation potential)
RESULTS OF THE LCA - INDICATORS TO DESCRIBE RESOURCE USE according to EN 15804+A2: 1 door closer
Parameter Unit A1-A3 A4 A5 C1 C2 C3 C4 D
PERE MJ 1.84E+01 6E-03 1.34E+00 0 3.04E-04 2.01E-01 0 -1.6E+01
PERM MJ 1.48E+00 0 -1.33E+00 0 0 -1.52E-01 0 0
PERT MJ 1.99E+01 6E-03 9E-03 0 3.04E-04 4.8E-02 0 -1.6E+01
PENRE MJ 1.35E+02 1.72E+00 5E-02 0 9.7E-02 3.09E+00 0 -3.93E+01
PENRM MJ 2.9E+00 0 0 0 0 -2.9E+00 0 0
PENRT MJ 1.38E+02 1.72E+00 5E-02 0 9.7E-02 1.87E-01 0 -3.93E+01
SM kg 9.52E-01 0 0 0 0 0 0 0
RSF MJ 0 0 0 0 0 0 0 0
NRSF MJ 0 0 0 0 0 0 0 0
FW m3 6.3E-02 9.94E-06 4.59E-04 0 5.46E-07 1E-03 0 -2.8E-02
PERE = Use of renewable primary energy excluding renewable primary energy resources used as raw materials; PERM = Use of renewable primary
energy resources used as raw materials; PERT = Total use of renewable primary energy resources; PENRE = Use of non-renewable primary energy
excluding non-renewable primary energy resources used as raw materials; PENRM = Use of non-renewable primary energy resources used as raw
materials; PENRT = Total use of non-renewable primary energy resources; SM = Use of secondary material; RSF = Use of renewable secondary fuels;
NRSF = Use of non-renewable secondary fuels; FW = Use of net fresh water
RESULTS OF THE LCA – WASTE CATEGORIES AND OUTPUT FLOWS according to EN 15804+A2:
1 door closer
Parameter Unit A1-A3 A4 A5 C1 C2 C3 C4 D
HWD kg 7.74E-06 1.68E-10 7.32E-11 0 9.37E-12 6.96E-10 0 -3.82E-08
NHWD kg 1.5E+00 1.76E-04 5E-03 0 9.88E-06 4.1E-02 0 -6.22E-01
RWD kg 1.79E-03 1.88E-06 2.61E-06 0 1.04E-07 7.03E-06 0 -4E-03
CRU kg 0 0 0 0 0 0 0 0
MFR kg 0 0 0 0 0 1.46E+00 0 0
MER kg 0 0 0 0 0 0 0 0
EEE MJ 0 0 2.38E-01 0 0 0 0 0
EET MJ 0 0 4.32E-01 0 0 0 0 0
HWD = Hazardous waste disposed; NHWD = Non-hazardous waste disposed; RWD = Radioactive waste disposed; CRU = Components for re-use;
MFR = Materials for recycling; MER = Materials for energy recovery; EEE = Exported electrical energy; EET = Exported thermal energy
4 Environmental Product Declaration - dormakaba - TS 71/TS 72
RESULTS OF THE LCA – additional impact categories according to EN 15804+A2-optional:
1 door closer
Parameter Unit A1-A3 A4 A5 C1 C2 C3 C4 D
Disease
PM 1.56E-06 3.62E-08 2.44E-10 0 3.58E-11 9.07E-10 0 -1.6E-07
incidence
IR kBq U235 eq 1.99E-01 2.69E-04 4.04E-04 0 1.48E-05 6.52E-04 0 -7.81E-01
ETP-fw CTUe 4.82E+01 1.22E+00 2.4E-02 0 6.8E-02 7E-02 0 -1.4E+01
HTP-c CTUh 4.9E-09 2.29E-11 1.25E-12 0 1.29E-12 6.05E-12 0 -1.09E-09
HTP-nc CTUh 1.5E-07 1.02E-09 5.4E-11 0 5.5E-11 6.03E-10 0 3E-10
SQP SQP 3.41E+01 4E-03 1.3E-02 0 2.48E-04 5.6E-02 0 -1.57E+00
PM = Potential incidence of disease due to PM emissions; IR = Potential Human exposure efficiency relative to U235; ETP-fw = Potential comparative
Toxic Unit for ecosystems; HTP-c = Potential comparative Toxic Unit for humans (cancerogenic); HTP-nc = Potential comparative Toxic Unit for humans
(not cancerogenic); SQP = Potential soil quality index
Disclaimer 1 – for the indicator “Potential Human exposure efficiency relative to U235”. This impact category deals mainly with the
eventual impact of low-dose ionizing radiation on human health of the nuclear fuel cycle. It does not consider effects due to possible
nuclear accidents, occupational exposure or radioactive waste disposal in underground facilities. Potential ionizing radiation from the
soil, radon and from some construction materials is also not measured by this indicator.
Disclaimer 2 – for the indicators “abiotic depletion potential for non-fossil resources”, “abiotic depletion potential for fossil resources”,
“water (user) deprivation potential, deprivation-weighted water consumption”, “potential comparative toxic unit for ecosystems”,
“potential comparative toxic unit for humans – cancerogenic”, “Potential comparative toxic unit for humans - not cancerogenic”,
“potential soil quality index”. The results of this environmental impact indicator shall be used with care as the uncertainties on these
results are high as there is limited experience with the indicator.
References
EN 1154 GaBi
EN 1154-2003; Building hardware - Controlled door closing Sphera Solutions GmbH Gabi Software System and Database
devices - Requirements and test methods for Life Cycle Engineering 1992-2020 Version 10.0.0.71
University of Stuttgart Leinfelden-Echterdingen
EN 1634-1
EN 1634-1:2018; Fire resistance and smoke control tests for GaBi ts documentation
door and shutter assemblies, openable windows and elements GaBi life cycle inventory data documentation (https://www.gabi-
of building hardware - Part 1: Fire resistance test for door and software.com/support/gabi/gabidatabase- 2020-lci-
shutter assemblies and openable windows documentation/)
ISO 14025 LCA-tool dormakaba
DIN EN ISO 14025:2011-10, Environmental labels and LCA tool IBU-DOR-202104-LT1-EN, version 1.0, 2021.
declarations — Type III environmental declarations — Developed by Sphera Solutions GmbH
Principles and procedures
PCR Part A
EN 15804 PCR – Part A: Calculation Rules for the Life Cycle Assessment
EN 15804+A2:2019+AC:2021, Sustainability of construction and Requirements on the Project Re-port according to EN
works — Environmental Product Declarations — Core rules for 15804+A2:2019, Version 1.0, 2020, Institut Bauen und Umwelt
the product category of construction products e.V., www.ibu-epd.com
REACH Regulation PCR Part B
Regulation (EC) No 1907/2006 of the European Parliament and PCR – Part B: Requirements on the EPD for Building Hardware
of the Council on the Registration, Evaluation, Authorisation product, version 1.2, Institut Bauen und Umwelt e.V., www.ibu-
and Restriction of Chemicals (REACH) epd.com, 2017
Further References
IBU
Institut Bauen und Umwelt e.V.: General Instructions for the
EPDs programme of Institut Bauen und Umwelt e.V. Version
2.0., Berlin: Institut Bauen und Umwelt e.V., 2021. www.ibu-
epd.com
5 Environmental Product Declaration - dormakaba - TS 71/TS 72
Publisher
Institut Bauen und Umwelt e.V. +49 (0)30 3087748- 0
Hegelplatz 1 info@ibu-epd.com
10117 Berlin www.ibu-epd.com
Germany
Programme holder
Institut Bauen und Umwelt e.V. +49 (0)30 3087748- 0
Hegelplatz 1 info@ibu-epd.com
10117 Berlin www.ibu-epd.com
Germany
Author of the Life Cycle Assessment
Sphera Solutions GmbH +49 711 341817-0
Hauptstraße 111- 113 info@sphera.com
70771 Leinfelden-Echterdingen www.sphera.com
Germany
Owner of the Declaration
dormakaba International Holding GmbH +49 2333 793-0
DORMA Platz 1 info.de@dormakaba.com
58256 Ennepetal www.dormakaba.com
Germany
6 Environmental Product Declaration - dormakaba - TS 71/TS 72
