ENVIRONMENTAL PRODUCT DECLARATION
as per ISO 14025 and EN 15804+A2
Owner of the Declaration Tapibel NV
Publisher Institut Bauen und Umwelt e.V. (IBU)
Programme holder Institut Bauen und Umwelt e.V. (IBU)
Declaration number EPD-TAP-20240098-IBA1-EN
Issue date 30.07.2024
Valid to 29.07.2029
TUFTED CARPET TILES with total pile weight between 485 and
1300 g/m², solution-dyed yarn, pile material virgin polyamide 6,
modified bitumen backing with 70 % recycled content
Tapibel NV
www.ibu-epd.com | https://epd-online.com
1. General Information
Tapibel NV TUFTED CARPET TILES with total pile weight
between 485 and 1300 g/m², solution-dyed yarn,
pile material virgin polyamide 6, modified bitumen
backing with 70 % recycled content
Programme holder Owner of the declaration
IBU – Institut Bauen und Umwelt e.V. Tapibel NV
Hegelplatz 1 Industrielaan 4
10117 Berlin 3900 Pelt
Germany Belgium
Declaration number Declared product / declared unit
EPD-TAP-20240098-IBA1-EN 1 m² installed tufted carpet tiles with a pile of solution-dyed virgin
polyamide 6 and a modified bitumen backing with 70 % recycled content
This declaration is based on the product category rules: Scope:
Floor coverings, 01.08.2021 The manufacturer declaration applies to a group of similar products with a
(PCR checked and approved by the SVR) total pile weight varying between 485 and 1300 g/m². The results given in
the EPD correspond to tufted carpet tiles with a pile weight of 525 g/m².
LCA results for product groups having a minimum pile weight of 485 g/m²,
Issue date an intermediate pile weight of 800 g/m² or a maximum pile weight of 1300
g/m² can be taken from the corresponding tables of the annexe.
30.07.2024
The products are manufactured in the production sites at Pelt, Belgium
(tufting), and Nijkerk, The Netherlands (back coating).
Valid to
29.07.2029 The owner of the declaration shall be liable for the underlying information
and evidence; the IBU shall not be liable with respect to manufacturer
information, life cycle assessment data and evidences.
The EPD was created according to the specifications of EN 15804+A2. In
the following, the standard will be simplified as EN 15804.
Verification
The standard EN 15804 serves as the core PCR
Independent verification of the declaration and data according to ISO
14025:2011
Dipl.-Ing. Hans Peters internally X externally
(Chairman of Institut Bauen und Umwelt e.V.)
Florian Pronold Angela Schindler,
(Managing Director Institut Bauen und Umwelt e.V.) (Independent verifier)
Environmental Product Declaration - Tapibel NV - TUFTED CARPET TILES with total pile weight between 485 and 1300 g/m², solution-dyed yarn, pile material virgin
1 polyamide 6, modified bitumen backing with 70 % recycled content
2. Product
Performance data of the product are in accordance with the
2.1 Product description/Product definition declaration of performance with respect to its essential
Tufted carpet tiles having a pile of solution-dyed virgin characteristics according to EN 14041: 2018-05, Resilient,
polyamide 6, a precoat based on recycled polyvinyl butyral textile and laminate floor coverings - Essential characteristics.
(PVB) and a modified bitumen backing system with recycled Additional product properties can be found on the
filler. manufacturer's website (www.tapibel.be).
For tufted carpet tiles with a pile weight between 485 and 1300 2.4 Delivery status
g/m², the recycled content (i.e. PVB in the precoat and Typical dimensions of tufted carpet tiles are 50 x 50 cm, but
limestone filler in the bitumen backing) varies between 51 % also other dimensions (25 x 100 cm, 100 x 100 cm, 100 x 200
and 43 %, depending on the amount of the virgin polyamide 6 cm) are possible.
yarns in the pile. The recycled content of the bitumen backing
itself is 70 %. 2.5 Base materials/Ancillary materials
Name Value Unit
The declaration applies to a group of products with a pile polyamide 6 (low carbon footprint (CFP) grades) 12 %
weight varying between 485 and 1300 g/m². The LCA results
polyester/polyethylene 2 %
are calculated for products with a pile weight of 525 g/m². LCA
polypropylene 1 %
results for product groups having a minimum (485 g/m²),
intermediate (800 g/m²) or maximum (1300 g/m²) pile weight limestone (partly recycled) 61 %
can be taken from the corresponding tables of the annexe. polyvinyl butyral (recycled) 3 %
bitumen 18 %
For the placing on the market of the specific product in the
glass fiber 1 %
European Union/European Free Trade Association (EU/EFTA)
additives 2 %
(with the exception of Switzerland), Regulation (EU) No.
305/2011 Construction Product Regulation (CPR) applies. The
product needs a Declaration of Performance (DoP) taking into The recycled content of the tufted carpet tiles with a pile weight
consideration EN 14041:2018-05, Resilient, textile and laminate between 485 and 1300 g/m² varies between 51 % and 43 %,
floor coverings - Essential characteristics, and the CE-marking. depending on the amount of the virgin polyamide 6 yarns in the
The DoP of the product can be found on the manufacturer's pile. The recycled content of the bitumen backing itself is 70 %.
technical information section (www.tapibel.be). For the
application and use of the product, the respective national The PA6 yarn, used in the tufted carpet tiles considered in this
provisions apply. LCA study, is a low-impact PA6 carpet yarn that is based on the
most recent innovations in polymer production. It only uses low
2.2 Application carbon footprint (CFP) polyamide grades from suppliers who
The products can be used as a floor covering in both residential calculated their specific carbon footprint.
and commercial buildings. According to the use class as
defined in EN 1307, the products can be used in all commercial The specific product covered by the EPD contains substances
areas which require class 33 or less. listed in the ECHA candidate list (date: 26.07.2022) exceeding
0.1 percentage by mass: no
This product contains other carcinogenic, mutagenic, reprotoxic
(CMR) substances in categories 1A or 1B which are not on the
candidate list, exceeding 0.1 percentage by mass: no
Biocide products were added to this construction product or it
has been treated with biocide products (this then concerns a
treated product as defined by the (EU) Ordinance on
BiocideProducts No. 528/2012): no
2.3 Technical Data
Technical data are given in the following table:
Constructional data 2.6 Manufacture
For manufacturing of the tufted carpet tiles, the PA6 yarns are
Name Value Unit
first tufted on a primary backing and subsequently precoated
Modular carpet tiles 50 x 50 cm - also
with a latex-free compound. Then, the modified bitumen
Product Form other dimensions possible (e.g. 25 x 100 -
backing is applied. Once the backing is cooled down, the
cm)
material is cut into tiles and prepared for shipment.
Type of
Tufted tiles -
manufacture
Yarn type Virgin PA 6, solution-dyed -
Secondary Bitumen-based heavy backing with 70 %
-
backing recycled content
Total pile
525 Min. 485 Max. 1300 g/m²
weight
Total carpet
4425 Min. 4275 Max. 4925 g/m2
weight
Environmental Product Declaration - Tapibel NV - TUFTED CARPET TILES with total pile weight between 485 and 1300 g/m², solution-dyed yarn, pile material virgin
2 polyamide 6, modified bitumen backing with 70 % recycled content
2.7 Environment and health during manufacturing 2.13 Extraordinary effects
The production conditions do not demand any special Fire
health protection measures over and beyond the legal The reaction to fire is determined according to EN 13501-1. The
requirements. class for tufted carpet tiles produced by Tapibel is Bfl-S1.
2.8 Product processing/Installation Water
The tufted carpet tiles are either loosely laid upon the screed In case of a leak or a flood where the flooring has been soaked
without any additional fixation or glued onto the underlying for a longer period of time (days), the flooring will most probably
screed using a special glue. be considered a total loss. In case of short or shorter time of
exposure and after drying, no visible damage may be expected,
2.9 Packaging
except for some stains.
The tufted carpet tiles are packed in cardboard boxes, placed
on wooden pallets and wrapped in plastic film. Mechanical destruction
In case of more severe damage, the damaged carpet tiles can
2.10 Condition of use
be replaced. The damaged carpet tiles go into the normal end-
The substantial composition during the use phase refers to the
of-life treatment.
composition during manufacturing. The conditions of use are
described in the producer's documentation. 2.14 Re-use phase
Tufted carpet tiles, which are not at the end-of-life stage, may
2.11 Environment and health during use
be uninstalled and reused as a floor covering. Post-consumer
After the first year, no product-related volatile organic
carpet tiles waste can be (partly) recycled or incinerated with
compound (VOC) emissions are relevant due to known VOC
energy recovery at its end-of-life.
decay curves of the product.
2.15 Disposal
2.12 Reference service life
Post-installation and post-consumer tufted carpet tiles are
The service life of textile floor coverings strongly depends on
considered textile waste. The European Waste Code EWC is
the correct installation taking into account the declared use
20 01 11. Tufted carpet tiles can be incinerated with energy
classification and the adherence to cleaning and maintenance
recovery or landfilled at their end-of-life.
instructions. A calculation of the reference service life according
to ISO 15686 is not possible. Alternatively, a minimum service 2.16 Further information
life of 10 years can be assumed, during which the functional All information about the product composition, technical
and visual quality is guaranteed (based on BNB, performance, instructions for installation and maintenance,
Nutzungsdauer von Bauteilen, BBSR table). The technical precautionary instructions for use, CE marking and relevant
service life can be significantly longer. DoP (declaration of performance) documents on tufted carpet
tiles, produced by Tapibel NV, can be found on the
manufacturer's website (www.tapibel.be).
3. LCA: Calculation rules
3.1 Declared Unit 3.2 System boundary
The declared unit refers to 1 m² textile floor covering consisting Type of EPD
of tufted carpet tiles with a pile of 525 g/m² solution-dyed virgin Cradle-to-gate with options: modules A1-A3, module C1-C4 and
polyamide 6 and a modified bitumen backing with 70 % module D and additional modules A4, A5, B1, B2.
recycled content.
System boundaries of modules A, B, C, D
The recycled content of these tufted carpet tiles is 50 %. Modules C2, C3, C4 and D are indicated separately for three
end-of-life scenarios:
The output of modules A1 to A3 corresponds to 1 m² produced 1 - landfill disposal
tufted carpet tiles, including production losses. 2 - municipal waste incineration
3 - recovery in the cement industry
The output of module A5 corresponds to 1 m² installed tufted
carpet tiles. In this module, an extra 3% production and A1-A3 Production
transport of tufted carpet tiles due to losses during installation, Energy and water consumption and supply, production of the
as well as final treatment of the installation and packaging basic material, processing of secondary material, auxiliary
waste are considered. material, packaging material, transport of the material and
packaging to the manufacturing site, infrastructure and land
use, waste water treatment and waste processing or final waste
disposal. For the modelling of the PA6 yarns, verified LCA data
Declared unit and mass reference
from the supplier has been used. Biogenic carbon that is stored
Name Value Unit
in renewable packaging material (cardboard and wooden
Declared unit 1 m2 pallets) is taken into account. Both the associated carbon
Conversion factor to 1 kg 0.226 dioxide uptake from the air during its production and the
Grammage 4.425 kg/m2 release of this carbon dioxide into the air during its final waste
treatment are considered. Generated electricity and steam due
Layer thickness 0.007 m
to the incineration of production waste and packaging waste
Other declared units are allowed if the conversion is shown are listed in the result table as exported energy.
transparently.
Environmental Product Declaration - Tapibel NV - TUFTED CARPET TILES with total pile weight between 485 and 1300 g/m², solution-dyed yarn, pile material virgin
3 polyamide 6, modified bitumen backing with 70 % recycled content
A4 Transport C3-3.
Transport of the packed textile floor covering from factory gate
to the place of installation. D Benefits and loads beyond the system boundaries
Calculated potential benefits result from materials exclusive
A5 Installation secondary materials (net primary materials).
Installation of the textile floor covering, processing of D-A5: Potential benefits and loads due to recycling and
installation waste and packaging waste up to energy and/or incineration of waste arising from final product packaging and
material recovery or final disposal, production of the amount of potential benefits for generated energy due to incineration of
tufted carpet tiles and their packaging that occurs as installation installation waste in a municipal waste incineration plant with
waste including the transport to the place of installation. The R1>0.6.
tufted carpet tiles are considered to be loosely laid upon the D-1: No potential benefits nor loads due to landfill disposal of
screed without using any additional materials or energy. If tufted carpet tiles waste at end-of-life.
attached to the floor instead, the necessary auxiliary materials D-2: Potential benefits for generated energy due to incineration
are not taken into account in this EPD. Furthermore, of tufted carpet tiles waste at end-of-life in a municipal waste
preparation of the floor is beyond the system boundaries and incineration plant with R1>0.6.
also not considered. Biogenic carbon that is stored in D-3: Potential benefits for saved fossil fuels and saved
renewable packaging material (cardboard and wooden pallets) inorganic material due to recovery of tufted carpet tiles waste in
is released as carbon dioxide emissions into the air at the end a cement plant at end-of-life.
of life in module A5. Generated electricity and steam due to the
incineration of installation and packaging waste are listed in the 3.3 Estimates and assumptions
result table as exported energy.
3.4 Cut-off criteria
B1 Use In the assessment, all available data from the production
Indoor emissions during the use stage. After the first year, no process are considered, i.e. all raw materials used, utilised
product-related volatile organic compound (VOC) emissions are thermal energy and electric power consumption using the best
relevant due to known VOC decay curves of the product. available LCI datasets. Thus, material and energy flows
contributing less than 1 % of mass or energy are also
B2 Maintenance considered. Only packaging of ancillary materials in module A3
Cleaning of the textile floor covering for a period of 1 year: is not considered due to the very low amounts, as well as
accidental pollution and environmental impacts caused by the
• Vacuum cleaning – electricity supply
personnel of the production plants.
• Wet cleaning – electricity, water consumption,
production of the cleaning agent, waste water treatment 3.5 Background data
The declared values in this module have to be multiplied by the Background data are taken from the Ecoinvent v3.8 Cut-off and
assumed service life of the floor covering in the building in the Industry Data 2.0 databases.
question.
3.6 Data quality
B3-B5 The used data refer to the year 2021. The data for the
The modules are not relevant within the assumed reference foreground processes are based on input-output analyses at
service life of 10 years and are thus not declared. the Belgian and Dutch production sites of the here considered
tufted carpet tiles. The primary data collection was done
B6-B7 thoroughly, all flows have been considered. For modelling
No energy and water input are required for the operation of the foreground and background data, the Ecoinvent v3.8 Cut-off
carpet tiles in the use stage. The modules are not relevant and and Industry Data 2.0 databases have been used. Data quality
not declared. of foreground data is good for the most relevant flows, although
proxies had to be used for some inputs due to lack of specific
C1 Deconstruction data records. Furthermore, for modelling of the PA6 yarns, the
The floor covering is deconstructed manually and no additional results from the verified LCA study provided by the
environmental impact is caused. manufacturer of the yarns have been used. These results are
partly based on data delivered by the PA6 manufacturers and
C2 Transport partly on generic datasets. For background data, relevant
C2-1: Transport of the tufted carpet tiles waste to a landfill. Ecoinvent v3.8 data records have been used. The data quality
C2-2: Transport of the tufted carpet tiles waste to a municipal can be considered as good.
waste incineration plant (MWI).
C2-3: Transport of the tufted carpet tiles waste to a cement 3.7 Period under review
plant for recovery in the cement industry. The period under review is 2021.
3.8 Geographic Representativeness
C3 Waste processing
C3-1: Landfill disposal needs no waste processing. Land or region, in which the declared product system is
C3-2: Impact from waste incineration in a municipal waste manufactured, used or handled at the end of the product´s
incineration plant with R1>0.6. Generated electricity and steam lifespan: Belgium
are listed in the result table as exported energy.
C3-3: Impact from waste incineration in a cement kiln.
3.9 Allocation
Generated heat is listed in the result table as exported energy.
At Tapibel NV, different types of carpet tiles are produced. Only
facility-level data were available for the use of electricity, natural
C4 Final disposal
gas, water and ancillary materials. The facility-level data have
C4-1: Impact from landfill disposal.
been allocated to the analysed product using its respective
C4-2: The tufted carpet tiles waste leaves the system in module
annual production volume, expressed in m².
C3-2.
C4-3: The tufted carpet tiles waste leaves the system in module
Environmental Product Declaration - Tapibel NV - TUFTED CARPET TILES with total pile weight between 485 and 1300 g/m², solution-dyed yarn, pile material virgin
4 polyamide 6, modified bitumen backing with 70 % recycled content
Background data are taken from the Ecoinvent v3.8 Cut-off and
3.10 Comparability the Industry Data 2.0 databases.
Basically, a comparison or an evaluation of EPD data is only
possible if all the data sets to be compared were created
according to EN 15804 and the building context, respectively
the product-specific characteristics of performance, are taken
into account.
4. LCA: Scenarios and additional technical information
Name Value Unit
Characteristic product properties of biogenic carbon
Maintenance cycle for vacuum cleaning 208 number/year
The tufted carpet tiles do not contain any biogenic carbon.
Maintenance cycle for wet cleaning 1.5 number/year
However, the accompanying packaging of both the raw
materials and the final product does contain biogenic carbon. Water consumption for wet cleaning 4.000 kg/year
Cleaning agent for wet cleaning 0.090 kg/year
Information on describing the biogenic carbon content at Electricity consumption for vacuum
0.314 kWh/year
factory gate cleaning and wet cleaning
1 kg biogenic carbon is equivalent to 44/12 kg of CO2. Waste water treatment for wet cleaning 4.000 kg/year
Name ValueUnit
kg
Biogenic carbon content in product -
C
Biogenic carbon content in accompanying kg Reference service life
0.106
packaging C
Name Value Unit
Reference service life
(according to BBSR table, BNB, 10 a
Transport to the construction site (A4) 2017)
Corresponds to the
Name Value Unit Declared product properties (at
specifications of EN -
Litres of fuel truck 16-32 ton EURO 6 0.0057 l/100km the gate) and finishes
1307
Transport distance 700 km
An assumed quality of work,
Capacity utilisation (including empty runs) 85 % when installed in accordance According to the
manufacturer's -
with the manufacturer’s
Installation in the building (A5) instructions
instructions
The tufted carpet tiles are considered to be loosely laid upon
Usage conditions, e.g. Use in areas defined by
the screed. This action does not require any materials nor
frequency of use, mechanical the use class according -
energy inputs or outputs. The preparation of the floor is beyond
exposure to EN 1307
the system boundaries and thus not taken into account.
Maintenance e.g. required According to the
frequency, type and quality and manufacturer's -
The installation losses are considered to be incinerated in a
replacement of components instructions
municipal waste incineration plant with R1>0.6.
End of Life (C1-C4)
Packaging waste is considered to be treated according to
Three different end-of-life scenarios are declared and the
European default scenarios for packaging waste (Eurostat,
results are indicated separately in module C. Each scenario is
2020). This treatment includes landfill, incineration in a
calculated as a 100 % scenario:
municipal waste incineration plant with R1<0.6 and/or recycling.
• Scenario 1: 100 % landfill disposal;
Name Value Unit • Scenario 2: 100 % municipal waste incineration (MWI)
with R1>0,6;
Material loss 0.133 kg
• Scenario 3: 100 % recovery in the cement industry.
Maintenance (B2)
If combinations of these scenarios have to be calculated, this
The values for cleaning refer to 1 m² floor covering per year.
should be done according to the following scheme:
Depending on the application based on ISO 10874, the
technical service life recommended by the manufacturer and
EOL impact = x % impact (Scenario 1) + y % impact (Scenario
the anticipated strain on the floor by customers, the case-
2) + z % impact (Scenario 3) with x % + y % + z % = 100 %.
specific useful life can be established. Based on this useful life,
the effects of module B2 need to be calculated in order to
Waste transport (C2)
obtain the overall environmental impacts.
Waste is transported to its waste treatment using a truck, 16-32
tons, EURO 6. The transport distances vary between waste
For further information on cleaning and maintenance, see
treatment:
www.tapibel.be.
• Scenario 1: transport to a landfill: 50 km
Scenario 2: transport to a waste incineration plant: 150
km
• Scenario 3: transport to a cement plant for recovery in
the cement industry: 200 km
Environmental Product Declaration - Tapibel NV - TUFTED CARPET TILES with total pile weight between 485 and 1300 g/m², solution-dyed yarn, pile material virgin
5 polyamide 6, modified bitumen backing with 70 % recycled content
Reuse, recovery and/or recycling potentials (D), relevant
Waste processing (C3)
scenario information
Waste processing varies according to waste treatment
Recovery or recycling potentials due to the three end-of-life
scenario:
scenarios (module C) are indicated separately.
• Waste incineration (scenario 2): The organic material
within the tufted carpet tiles is considered to be Here, calculated potential benefits result from materials,
incinerated. The ashes of the inorganic material within exclusive secondary materials (net primary materials).
the tufted carpet tiles are considered to be landfilled.
• Recovery in the cement industry (scenario 3): The Recovery in the cement industry (scenario 3): The organic
organic material within the tufted carpet tiles is material of the tufted carpet tiles is considered to be used as an
considered to be incinerated and to serve as a alternative fuel in a cement kiln. It mainly substitutes for lignite
secondary fuel in the cement kiln. The inorganic material (68.8 %), hard coal (23.6 %) and petrol coke (7.6 %) (VDZ e.V.,
within the tufted carpet tiles is considered to be 2020). The avoided production of these fossil fuels as well as
integrated in the cement clinker and to substitute for the the avoided emissions due to incineration of these fossil fuels
original raw material input. are accounted for in module D, taking into account the lower
heating values of the fuels and the organic material in the
carpet tiles. The inorganic material is considered to be
Name ValueUnit
substantially integrated into the cement clinker and to substitute
Collected as mixed construction waste (scenario 1
4.425 kg for the original material input. The avoided production of the
and scenario 2)
original primary raw material is accounted for in module D.
Collected separately waste type (scenario 3) 4.425 kg
Name Value Unit
Landfilling (scenario 1) 4.425 kg
Energy recovery in cement industry 1.573 kg
Energy recovery (scenario 2) 4.425 kg
Recycling in cement industry 0.681 kg
Energy recovery in cement industry (scenario 3 -
1.713 kg
accounted for in module D3)
Recycling in cement industry (scenario 3 -
2.712 kg
accounted for in module D3)
Environmental Product Declaration - Tapibel NV - TUFTED CARPET TILES with total pile weight between 485 and 1300 g/m², solution-dyed yarn, pile material virgin
6 polyamide 6, modified bitumen backing with 70 % recycled content
5. LCA: Results
The LCA results are valid for 1 m² tufted carpet tiles with a pile of 525 g/m² solution-dyed virgin polyamide 6 and a modified bitumen
backing with 70 % recycled content.
The output of modules A1 to A3 corresponds to 1 m² produced tufted carpet tiles, including production losses. The output of module A5
corresponds to 1 m² installed tufted carpet tiles. In this module, an extra 3% production and transport of tufted carpet tiles due to losses
during installation, as well as final treatment of the installation and packaging waste are considered.
The result figures given in module B2 refer to a period of 1 year, because a reference service life is not declared. They have to be
multiplied by the assumed service life (in years) of the floor covering in the building under consideration.
The modules C3/1, C4/2 and C4/3 cause no additional impact and are thus set to zero (see chapter "LCA: Calculation rules").
The values in column D result from module A5.
The EF3.0 characterisation factors from EC-JRC have been applied.
DESCRIPTION OF THE SYSTEM BOUNDARY (X = INCLUDED IN LCA; MND = MODULE OR INDICATOR NOT DECLARED; MNR
= MODULE NOT RELEVANT)
Benefits and
Construction loads beyond
Product stage Use stage End of life stage
process stage the system
boundaries
la ire ta m w a Ry lp p u s tro p s n a rT g n iru tc a fu n a M e h t m o rf tro p s n a rTe tis e h t o t e ta g y lb m e s s A e s U e c n a n e tn ia M ria p e R tn e m e c a lp e R tn e m h s ib ru fe R y g re n e la n o ita re p Oe s u re ta w la n o ita re p Oe s u n o itc u rts n o c -e Dn o itilo m e d tro p s n a rT g n is s e c o rp e ts a W la s o p s iD -e s u e R-y re v o c e R-g n ilc y c e Rla itn e to p
A1 A2 A3 A4 A5 B1 B2 B3 B4 B5 B6 B7 C1 C2 C3 C4 D
X X X X X X X MNR MNR MNR MND MND X X X X X
RESULTS OF THE LCA - ENVIRONMENTAL IMPACT according to EN 15804+A2: 1 m² installed tufted carpet tiles with a pile of
solution-dyed virgin polyamide 6 and a modified bitumen backing with 70 % recycled content
A1-
Parameter Unit A4 A5 B1 B2 C1 C2/1 C2/2 C2/3 C3C3/1 C3/2 C3/3 C4 C4/1 C4/2C4/3 D D/1 D/2 D/3
A3
GWP-total kg CO 2 4.33E 5.26E-5.76E- 0 2.64E- 0 3.61E-1.08E-1.44E- 0 0 4.04E 4.02E 0 2.52E- 0 0 -1.55E- 0 -1.19E -7.83E
eq +00 01 01 01 02 01 01 +00 +00 01 01 +00 +00
GWP-fossil kg CO 2 4.6E 5.25E- 2.9E- 0 2.63E- 0 3.6E- 1.08E-1.44E- 0 0 4.03E 4.01E 0 2.45E- 0 0 -6.24E- 0 -1.19E -7.83E
eq +00 01 01 01 02 01 01 +00 +00 01 02 +00 +00
GWP- kg CO 2 -2.78E-1.88E-2.86E- 0 1.12E- 0 1.29E-3.87E-5.16E- 0 0 6.79E-6.65E- 0 6.72E- 0 0 -9.28E- 0 -3.09E--2.64E-
biogenic eq 01 04 01 03 05 05 05 03 03 03 02 03 03
GWP-luluc kg CO 2 1.21E- 2.1E- 3.77E- 0 3.78E- 0 1.44E-4.32E-5.76E- 0 0 6.87E-6.31E- 0 1.65E- 0 0 -1.74E- 0 -1.23E--1.79E-
eq 02 04 04 04 05 05 05 05 05 05 04 03 03
kg
2.08E- 1.22E-7.04E- 2.11E- 8.35E- 2.5E- 3.34E- 3.03E-2.19E- 1.38E- -6.97E- -1.27E--1.05E-
ODP CFC11 0 0 0 0 0 0 0 0
06 07 08 08 09 08 08 08 08 08 09 07 07
eq
mol H+ 1.94E- 1.49E-7.23E- 1.71E- 1.02E-3.07E-4.09E- 1.23E-1.03E- 3.91E- -2.08E- -3.31E--3.03E-
AP 0 0 0 0 0 0 0 0
eq 02 03 04 03 04 04 04 03 03 04 04 03 02
EP- 1.07E- 3.75E-3.25E- 2.08E- 2.57E-7.71E-1.03E- 2.24E-2.04E- 4.15E- -3.61E- -5.56E--9.81E-
kg P eq 0 0 0 0 0 0 0 0
freshwater 03 06 05 05 07 07 06 06 06 07 06 05 04
7.73E- 2.97E-2.75E- 3.04E- 2.03E- 6.1E- 8.13E- 4.67E-3.94E- 3.1E- -4.26E- -5.19E--4.46E-
EP-marine kg N eq 0 0 0 0 0 0 0 0
03 04 04 04 05 05 05 04 04 04 05 04 03
mol N 4.52E- 3.31E-1.81E- 2.56E- 2.27E- 6.8E- 9.07E- 5.11E- 4.3E- 1.36E- -4.74E- -5.88E--4.93E-
EP-terrestrial 0 0 0 0 0 0 0 0
eq 02 03 03 03 04 04 04 03 03 03 04 03 02
kg
1.4E- 1.27E-5.63E-2.23E-8.62E- 8.71E-2.61E-3.48E- 1.34E- 1.11E- 4.41E- -1.61E- -1.74E--2.62E-
POCP NMVOC 0 0 0 0 0 0 0
02 03 04 04 04 05 04 04 03 03 04 04 03 02
eq
kg Sb 1.24E- 1.42E-4.65E- 2.01E- 9.76E-2.93E- 3.9E- 3.92E-3.43E- 8.73E- -3.77E- -3.89E--7.84E-
ADPE 0 0 0 0 0 0 0 0
eq 05 06 07 06 08 07 07 07 07 08 08 07 07
1.38E 7.97E 4.64E 7.31E 5.46E- 1.64E 2.19E 1.29E 6.84E- 1.01E -1.17E -2.26E -5.7E
ADPF MJ 0 0 0 0 0 0 0 0
+02 +00 +00 +00 01 +00 +00 +00 01 +00 +00 +01 +01
m3
9.48E- 2.43E-3.13E- 1.22E- 1.66E-4.99E-6.65E- 4.08E-3.79E- 1.23E- -8.91E- -1.25E--2.29E-
WDP world eq 0 0 0 0 0 0 0 0
01 02 02 01 03 03 03 02 02 02 03 01 01
deprived
GWP = Global warming potential; ODP = Depletion potential of the stratospheric ozone layer; AP = Acidification potential of land and water; EP =
Eutrophication potential; POCP = Formation potential of tropospheric ozone photochemical oxidants; ADPE = Abiotic depletion potential for non-fossil
resources; ADPF = Abiotic depletion potential for fossil resources; WDP = Water (user) deprivation potential)
Environmental Product Declaration - Tapibel NV - TUFTED CARPET TILES with total pile weight between 485 and 1300 g/m², solution-dyed yarn, pile material virgin
7 polyamide 6, modified bitumen backing with 70 % recycled content
RESULTS OF THE LCA - INDICATORS TO DESCRIBE RESOURCE USE according to EN 15804+A2: 1 m² installed tufted carpet
tiles with a pile of solution-dyed virgin polyamide 6 and a modified bitumen backing with 70 % recycled content
A1-
ParameterUnit A4 A5 B1 B2 C1 C2/1 C2/2 C2/3 C3 C3/1 C3/2 C3/3 C4 C4/1 C4/2 C4/3 D D/1 D/2 D/3
A3
2.35E 1.12E- 2.3E 6.34E- 7.68E- 2.3E- 3.07E- 8.36E- 5.93E- 3.94E- -2.86E -1.96E -1.29E
PERE MJ 0 0 0 0 0 0 0 0
+01 01 +00 01 03 02 02 02 02 02 +00 +00 +00
2.6E -1.5E 8.51E-
PERM MJ 0 0 0 0 0 0 0 0 0 0 0 0 0 0 0 0 0 0
+00 +00 01
2.61E 1.12E- 7.93E- 6.34E- 7.68E- 2.3E- 3.07E- 8.36E- 5.93E- 3.94E- -2.01E -1.96E -1.29E
PERT MJ 0 0 0 0 0 0 0 0
+01 01 01 01 03 02 02 02 02 02 +00 +00 +00
1.33E 7.97E 5.96E 7.31E 5.46E- 1.64E 2.19E 4.99E 4.93E 1.01E -1.17E -2.26E -5.7E
PENRE MJ 0 0 0 0 0 0 0 0
+02 +00 +00 +00 01 +00 +00 +01 +01 +00 +00 +01 +01
4.87E -3.89E- -4.86E -4.86E 7.26E-
PENRM MJ 0 0 0 0 0 0 0 0 0 0 0 0 0 0 0 0
+01 03 +01 +01 03
1.82E 7.97E 5.95E 7.31E 5.46E- 1.64E 2.19E 1.29E 6.84E- 1.01E -1.17E -2.26E -5.7E
PENRT MJ 0 0 0 0 0 0 0 0
+02 +00 +00 +00 01 +00 +00 +00 01 +00 +00 +01 +01
2.19E 6.57E- 6.15E- 6.81E-
SM kg 0 0 0 0 0 0 0 0 0 0 0 0 0 0 0 0 0
+00 02 02 01
RSF MJ 0 0 0 0 0 0 0 0 0 0 0 0 0 0 0 0 0 0 0 0 0
NRSF MJ 0 0 0 0 0 0 0 0 0 0 0 0 0 0 0 0 0 0 0 0 0
2.74E- 7.93E- 9.86E- 4.49E- 5.44E- 1.63E- 2.18E- 2.44E- 1.69E- 1.22E- -5.26E- -9.26E- -7.17E-
FW m3 0 0 0 0 0 0 0 0
02 04 04 03 05 04 04 03 03 03 04 03 03
PERE = Use of renewable primary energy excluding renewable primary energy resources used as raw materials; PERM = Use of renewable primary
energy resources used as raw materials; PERT = Total use of renewable primary energy resources; PENRE = Use of non-renewable primary energy
excluding non-renewable primary energy resources used as raw materials; PENRM = Use of non-renewable primary energy resources used as raw
materials; PENRT = Total use of non-renewable primary energy resources; SM = Use of secondary material; RSF = Use of renewable secondary fuels;
NRSF = Use of non-renewable secondary fuels; FW = Use of net fresh water
RESULTS OF THE LCA – WASTE CATEGORIES AND OUTPUT FLOWS according to EN 15804+A2:
1 m² installed tufted carpet tiles with a pile of solution-dyed virgin polyamide 6 and a modified bitumen backing with 70 %
recycled content
A1-
ParameterUnit A4 A5 B1 B2 C1 C2/1 C2/2 C2/3 C3 C3/1 C3/2 C3/3 C4 C4/1 C4/2 C4/3 D D/1 D/2 D/3
A3
4.8E- 2.08E- 1.57E- 5.51E- 1.43E- 4.28E- 5.7E- 2.86E- 2.13E- 1.28E- -1.19E- -1.86E- -8.91E-
HWD kg 0 0 0 0 0 0 0 0
04 05 05 06 06 06 06 06 06 06 06 05 06
6.57E- 4.17E- 2.06E- 2.35E- 2.86E- 8.58E- 1.14E- 3.01E 2.97E- 4.43E -4.48E- -4.16E- -1.16E-
NHWD kg 0 0 0 0 0 0 0 0
01 01 01 02 02 02 01 +00 01 +00 03 02 01
8.78E- 5.38E- 2.96E- 2.17E- 3.69E- 1.11E- 1.48E- 6.3E- 2.41E- 6.46E- -4.81E- -8.8E- -6.76E-
RWD kg 0 0 0 0 0 0 0 0
04 05 05 05 06 05 05 06 06 06 06 05 05
CRU kg 0 0 0 0 0 0 0 0 0 0 0 0 0 0 0 0 0 0 0 0 0
6.41E- 6.34E- 2.71E
MFR kg 0 0 0 0 0 0 0 0 0 0 0 0 0 0 0 0 0 0
02 02 +00
MER kg 0 0 0 0 0 0 0 0 0 0 0 0 0 0 0 0 0 0 0 0 0
3.27E- 2.34E- 5.22E
EEE MJ 0 0 0 0 0 0 0 0 0 0 0 0 0 0 0 0 0 0
02 01 +00
6.54E- 4.68E- 1.04E 1.04E
EET MJ 0 0 0 0 0 0 0 0 0 0 0 0 0 0 0 0 0
02 01 +01 +01
HWD = Hazardous waste disposed; NHWD = Non-hazardous waste disposed; RWD = Radioactive waste disposed; CRU = Components for re-use;
MFR = Materials for recycling; MER = Materials for energy recovery; EEE = Exported electrical energy; EET = Exported thermal energy
RESULTS OF THE LCA – additional impact categories according to EN 15804+A2-optional:
1 m² installed tufted carpet tiles with a pile of solution-dyed virgin polyamide 6 and a modified bitumen backing with 70 %
recycled content
A1-
Parameter Unit A4 A5 B1 B2 C1 C2/1 C2/2 C2/3 C3 C3/1 C3/2 C3/3 C4 C4/1 C4/2 C4/3 D D/1 D/2 D/3
A3
Disease 1.73E- 4.22E- 8.15E- 1.19E- 2.89E- 8.68E- 1.16E- 1.16E- 7.27E- 7.3E- -2.71E- -8.88E- -6.04E-
PM 0 0 0 0 0 0 0 0
incidence 07 08 09 08 09 09 08 08 09 09 09 09 07
kBq 3.77E- 3.46E- 1.35E- 2.6E- 2.37E- 7.11E- 9.49E- 5.21E- 2.47E- 4.54E- -5.45E- -1.04E- -6.92E-
IR 0 0 0 0 0 0 0 0
U235 eq 01 02 02 02 03 03 03 03 03 03 03 01 02
8.16E 6.25E 3.03E 5.93E 4.29E- 1.29E 1.72E 6.89E 6.53E 1.07E -4.72E- -6.07E -1.8E
ETP-fw CTUe 0 0 0 0 0 0 0 0
+01 +00 +00 +00 01 +00 +00 +00 +00 +00 01 +00 +02
2.72E- 2.01E- 1.31E- 3.96E- 1.38E- 4.14E- 5.52E- 7.1E- 6.93E- 2.99E- -1.8E- -1.91E- -6.02E-
HTP-c CTUh 0 0 0 0 0 0 0 0
09 10 10 10 11 11 11 10 10 11 11 10 09
6.69E- 6.32E- 2.59E- 7.64E- 4.33E- 1.3E- 1.73E- 5.65E- 5.44E- 4.71E- -4.27E- -4.86E- -3.08E-
HTP-nc CTUh 0 0 0 0 0 0 0 0
08 09 09 09 10 09 09 09 09 10 10 09 07
5.62E 5.55E 2.1E 9.16E- 3.81E- 1.14E 1.52E 1.88E 2.96E- 2.59E -1.12E -1.74E -4.7E
SQP SQP 0 0 0 0 0 0 0 0
+01 +00 +00 01 01 +00 +00 +00 01 +00 +01 +00 +00
PM = Potential incidence of disease due to PM emissions; IR = Potential Human exposure efficiency relative to U235; ETP-fw = Potential comparative
Toxic Unit for ecosystems; HTP-c = Potential comparative Toxic Unit for humans (cancerogenic); HTP-nc = Potential comparative Toxic Unit for humans
(not cancerogenic); SQP = Potential soil quality index
Footnote: For the calculation of PERM and PENRM, both the incinerated and the recycled packaging material of the final product is de-
booked in module A5, while in module D, only the recycled proportion is declared. Furthermore, 3% losses are considered in module
A5.
Environmental Product Declaration - Tapibel NV - TUFTED CARPET TILES with total pile weight between 485 and 1300 g/m², solution-dyed yarn, pile material virgin
8 polyamide 6, modified bitumen backing with 70 % recycled content
Disclaimer 1 – for the indicator 'Potential Human exposure efficiency relative to U235'. This impact category deals mainly with the
eventual impact of low dose ionizing radiation on human health of the nuclear fuel cycle. It does not consider effects due to possible
nuclear accidents, occupational exposure or radioactive waste disposal in underground facilities. Potential ionizing radiation from the
soil, radon and from some construction materials is also not measured by this indicator.
Disclaimer 2 – for the indicators 'abiotic depletion potential for non-fossil resources', 'abiotic depletion potential for fossil resources',
'water (user) deprivation potential, deprivation-weighted water consumption', 'potential comparative toxic unit for ecosystems', 'potential
comparative toxic unit for humans – cancerogenic', 'Potential comparative toxic unit for humans - not cancerogenic', 'potential soil
quality index'. The results of this environmental impact indicator shall be used with care as the uncertainties on these results are high
as there is limited experience with the indicator.
6. LCA: Interpretation
All environmental impact categories are mainly determined by has to be paid that the results for module B2 are only valid for
the PA6 yarns, the bitumen and the non-woven tuft cloth in one year of use of the tufted carpet tiles. In practice, the results
module A1 and by the energy use, the infrastructure and the should be multiplied by the assumed service life (in years) of
internal transport in module A3. For the modelling of the PA6 the floor covering in the building under consideration.
yarns, verified LCA data from the supplier has been used. The Incineration of the tufted carpet tiles in a municipal waste
impact of module A4 (transport to installation site) is mainly due incineration plant (scenario 2) or in a cement kiln (scenario 3) at
to the rather large transport distance. The impact of module B2 their end-of-life has a large impact on the GWP-fossil and
(maintenance) with the cleaning agent and electricity GWP-total indicators, while the impact of landfilling (scenario 1)
consumption as the most impacting processes is comparable to is limited.
the impact of module A5 (installation with 3 % losses). Attention
7. Requisite evidence
7.1 VOC emissions
TÜV PROFiCERT certification for VOC emissions and Determination of the VOC and formaldehyde emissions of
formaldehyde tufted carpet tiles according to/compliance with AgBB-Scheme,
The tufted carpet tiles, produced by Tapibel NV, fulfil the criteria French VOC label (A+), DE-UZ 128 (Blue Angel), EU Ecolabel,
V1.2 of the TÜV PROFiCERT-product Interior certification. Belgian VOC regulation, LEED v4 (outside North America),
Austrian Ecolabel UZ 35, GUT / PRODIS, BREEAM Exemplary
level, MVV TB Annex 8+9 / ABG and Finnish M1 classification.
Testing was done by TFI Aachen GmbH, Charlottenburger Allee
41, 52068 Aachen, Germany, www.tfi-aachen.de. Testing
reports: 21-001249-01 (2021) and 22-000301-02 (2022).
AgBB 2018 evaluation on day 3
Name Value Unit
TVOC 0.089 mg/m³
SVOC 0.000 mg/m³
R value 0.257
VOC w/o LCI 0.000 mg/m³
carcinogenic 0.000 mg/m³
DIBt parameter formaldehyde 0.000 mg/m³
7.2 CE marking
CE labelling according to EN 14041: DOP 000553T-003.
8. References
EN 1307
DIN EN 1307: 2014+A1:2016+A2:2018-05: Textile floor EN 15804
coverings - Classification DIN EN 15804:2012+A2:2019 + AC:2021, Sustainability of
construction works — Environmental Product Declarations —
EN 13501-1 Core rules for the product category of construction products
DIN EN 13501-1:2019-05: Fire classification of construction
products and building elements - Part 1: Classification using EN 16810
data from reaction to fire tests DIN EN 16810: 2017-08: Resilient, textile and laminate floor
coverings – Environmental product declarations – Product
EN 14041 category rules
DIN EN 14041: 2018-05 and DIN EN 14041: 2008-05:
Resilient, textile and laminate floor coverings - Essential ISO 10874
characteristics DIN EN ISO 10874: 2012+A1:2021-04: Resilient, textile and
Environmental Product Declaration - Tapibel NV - TUFTED CARPET TILES with total pile weight between 485 and 1300 g/m², solution-dyed yarn, pile material virgin
9 polyamide 6, modified bitumen backing with 70 % recycled content
laminate floor coverings - Classification Ecoinvent LCI database
Wernet, G., Bauer, C., Steubing, B., Reinhard, J., Moreno-Ruiz,
ISO 14025 E., and Weidema, B., 2016, The ecoinvent database version 3
DIN EN /ISO 14025:2011-10/, Environmental labels and (part I): overview and methodology. The International Journal of
declarations — Type III environmental declarations — Life Cycle Assessment, [online] 21(9), pp.1218–1230. Available
Principles and procedures at: http://link.springer.com/10.1007/s11367-016-1087-8
ISO 14040 European Ecolabel
DIN EN ISO 14040:2006+A1:2020 Environmental European Commission,
management - Life cycle assessment - Principles and https://environment.ec.europa.eu/topics/circular-economy/eu-
framework ecolabel-home_en
ISO 14044 European Waste Code
DIN EN ISO 14044:2006+A1:2018+A2:2020 Environmental Commission of the European Communities, 2010, Guidance on
management - Life cycle assessment - Requirements and classification of waste according to EWC-Stat categories
guideline
Eurostat
ISO 15686 Packaging waste treatment statistics 2020
ISO 15686: Buildings and constructed assets - Service life
planning Finnish M1 classification
ISO 15686-1: 2011-05: Part 1: General principles and Emission classification of building materials in Finland,
framework https://cer.rts.fi/en/m1-emission-class-for-building-material/
ISO 15686-2: 2012-05: Part 2: Service life prediction
procedures French VOC label
ISO 15686-7: 2017-04: Part 7: Performance evaluation for Ministère Français de l'écologie, du développement durable,
feedback of service life data from practice des transports et du logement, 2013
ISO 15686-8: 2008-06: Part 8: Reference service life and
service-life estimation Regulation (EU) No. 305/2011 GUT / PRODIS
Product passport for carpets and rugs, https://gut-prodis.eu/en/
AgBB Scheme
AgBB Scheme, Eco Institut, https://www.eco- Industry Data 2.0 database
institut.de/en/portfolio/agbb-schema/ SimaPro, Industry data LCA library,
https://simapro.com/databases/industry-data-lca-library/
Austrian Ecolabel
Austrian Ecolabel for Products, LEED
www.umweltzeichen.at/en/products/start LEED rating system, www.usgbc.org/leed
BBSR MVV TB Annex 8+9 / ABG
Bundesinstitut für Bau-, Stadt- und Raumforschung (BBSR) im Technical building rules, Deutsche Institut für Bautechnik,
Bundesamt für Bauwesen und Raumordnung (BBR), Bonn www.dibt.de/en/we-offer/technical-building-rules/
Belgian VOC regulation PCR Part A
FOD Volksgezondheid, Veiligheid van de voedselketen en Product Category Rules for Building-Related Products and
Leefmilieu, 2014, Koninklijk besluit tot vaststelling van de Services Part A: Calculation Rules for the Life Cycle
drempelniveaus voor de emissies naar het binnenmilieu van Assessment and Requirements on the Project Report according
bouwproducten voor bepaalde beoogde gebruiken to EN 15804+A2:2019, V1.3, Berlin: Institut Bauen und Umwelt
e.V. (IBU), August 2022
Blue Angel / Blauer Engel
Blue Angel, www.blauer-engel.de/en PCR Part B
Product Category Rules for Building-Related Products and
BNB Services Part B: Requirements on the EPD for floor coverings,
Nutzungsdauer von Bauteilen, Bewertungssystem Nachhaltiges V1.2, Berlin: Institut Bauen und Umwelt e.V. (IBU), September
Bauen (BNB), Nutzungsdauer von Bauteilen, 2022
Bundesministerium des Inneren, für Bau und Heimat,
24.02.2017 REACH
Regulation (EC) No 1907/2006 of the European Parliament and
B-PCR of the Council of 18 December 2006 concerning the
FPS Health, Food chain safety and Environment, 2022, B-EPD Registration, Evaluation, Authorisation and Restriction of
– Construction product category rules, Complementary to NBN Chemicals (REACH), June 2017
EN 15804+A2, Version 18.10.2022
Regulation No. 305/2011
BREEAM Construction Products Regulation (CPR) of the European
BRE certification system for a sustainable built environment, Council and of the European Parliament, April 2011
https://bregroup.com/products/breeam/
SimaPro LCA software
ECHA candidate list Pré Consultants, 2023, SimaPro 9.5.0.1 [Computer Software].
Candidate List of substances of very high concern (SVHCs) for Amersfoort, The Netherlands
authorisation, last update 26.07.2022, European Chemicals
Agency (ECHA), Helsinki, Finland TÜV PROFiCERT certification
TÜV PROFiCERT certification, https://www.proficert.de
Environmental Product Declaration - Tapibel NV - TUFTED CARPET TILES with total pile weight between 485 and 1300 g/m², solution-dyed yarn, pile material virgin
10 polyamide 6, modified bitumen backing with 70 % recycled content
Association of German Cement Works, Ed. Environmental Data
VDZ e.V. of the German Cement Industry 2020
Environmental Product Declaration - Tapibel NV - TUFTED CARPET TILES with total pile weight between 485 and 1300 g/m², solution-dyed yarn, pile material virgin
11 polyamide 6, modified bitumen backing with 70 % recycled content
Publisher
Institut Bauen und Umwelt e.V. +49 (0)30 3087748- 0
Hegelplatz 1 info@ibu-epd.com
10117 Berlin www.ibu-epd.com
Germany
Programme holder
Institut Bauen und Umwelt e.V. +49 (0)30 3087748- 0
Hegelplatz 1 info@ibu-epd.com
10117 Berlin www.ibu-epd.com
Germany
Author of the Life Cycle Assessment
Enperas +32 3 376 00 19
Thorpark 8300 info@enperas.com
3600 Genk https://www.enperas.com/en/
Belgium
Owner of the Declaration
Tapibel NV +32 (0)11 80 48 50
Industrielaan 4 werner@tapibel.be
3900 Pelt www.tapibel.be
Belgium
Environmental Product Declaration - Tapibel NV - TUFTED CARPET TILES with total pile weight between 485 and 1300 g/m², solution-dyed yarn, pile material virgin
12 polyamide 6, modified bitumen backing with 70 % recycled content
