ENVIRONMENTAL PRODUCT DECLARATION
as per ISO 14025 and EN 15804+A2
Owner of the Declaration DuPont de Nemours (Luxembourg) s.à r.l.
Programme holder Institut Bauen und Umwelt e.V. (IBU)
Publisher Institut Bauen und Umwelt e.V. (IBU)
Declaration number EPD-DUP-20210184-IBC1-EN
Issue date 30.11.2021
Valid to 29.11.2026
DuPont™ Tyvek® Monolayer 80 (1580B, 2480B)
DuPont de Nemours (Luxembourg) s.à r.l.
www.ibu-epd.com | https://epd-online.com
Umwelt Produktdeklaration Name des Herstellers – Name des Produkts
1. General Information
DuPont de Nemours (Luxembourg) s.à r.l. DuPont™ Tyvek® Monolayer 80
(1580B, 2480B)
Programme holder Owner of the declaration
IBU – Institut Bauen und Umwelt e.V. DuPont de Nemours (Luxembourg) s.à r.l.
Panoramastr. 1 Rue Général Patton
10178 Berlin L-2984 Contern
Germany Luxembourg
Declaration number Declared product / declared unit
EPD-DUP-20210184-IBC1-EN 1 m² DuPont™ Tyvek® Monolayer 80 (1580B, 2480B)
This declaration is based on the product Scope:
category rules: This document applies to DuPont™ Tyvek® 1580B
False ceiling and underlay sheeting, 11.2017 and 2480B monolayer high density polyethylene
(PCR checked and approved by the SVR) (HDPE) membranes manufactured by DuPont in L-
2984 Contern and printed in Germany, with a declared
unit weight of 81 g/m2. The LCA data were compiled
Issue date
using production data from the year 2019 by DuPont
30.11.2021
Luxembourg s.à r.l. The declaration holder is
responsible for the underlying data and its verification.
Valid to
29.11.2026
The owner of the declaration shall be liable for the
underlying information and evidence; the IBU shall not
be liable with respect to manufacturer information, life
cycle assessment data and evidences.
The EPD was created according to the specifications
of EN 15804+A2. In the following, the standard will be
simplified as EN 15804.
Verification
The standard EN 15804 serves as the core PCR
Independent verification of the declaration and data
according to ISO 14025:2010
Dipl. Ing. Hans Peters internally x externally
(chairman of Institut Bauen und Umwelt e.V.)
Dr. Alexander Röder Vito D'Incognito
(Managing Director Institut Bauen und Umwelt e.V.)) (Independent verifier)
2. Product
2.1 Product description/Product definition installed below Tyvek® is kept dry and performs as
DuPont™ Tyvek® is a nonwoven material made of designed.
HDPE, which is diffusion open but watertight. It is used
as a roof and wall underlay. 2.3 Technical Data
For the placing on the market of the product in the The following chapter comprises technical data for the
European Union/European Free Trade Association characteristics listed in the Declaration of Performance
(EU/EFTA) (with the exception of Switzerland) according to the harmonized technical specifications
Regulation (EU) No. 305/2011 (CPR) applies. The EN 13859-1 and EN 13859-2.
product needs a declaration of performance taking into
consideration EN 13859-1:2010 Flexible sheets for Technical Data
waterproofing - Definitions and characteristics of Name Value Unit
underlays - Part 1: Underlays for discontinuous roofing 50m
Length acc. to EN 1848-2 m
and EN 13859-2:2010 Flexible sheets for standard
waterproofing - Definitions and characteristics of 1.5m
Width acc. to EN 1848-2 m
underlays - Part 2 Underlays for walls and the CE- standard
marking. For the application and use the respective Grammage acc. to EN 1849-2 0.081 kg/m2
national provisions apply. Resistance to water penetration
W1 -
2.2 Application acc. to EN 1928 (class)
Tyvek® underlays are used in roofs and walls. They Water vapor diffusion equivalent
constitute the second water shedding layer and at the air layer thickness acc. to EN ISO 0.025 m
same time protect the insulation from trapped 12572
moisture, wind penetration, dust and insects. Insulation
2 Environmental Product Declaration DuPont de Nemours (Luxembourg) s.à r.l. – Tyvek® Monolayer 80 (1580B, 2480B)
Maximum tensile force acc. to EN stretch film. Vertical sides of the pallets are protected
250/210 N/50mm
12311-1 with a carton profile.
Elongation acc. to EN 12311-1 10/15 % All packaging materials can be reused (e.g. pallets),
Resistance to water penetration recycled or valorised through energy recovery.
after ageing acc. to EN 1297, EN W1 -
1928 (class)
Tear resistance (nail) acc. to EN 2.10 Condition of use
90/85 N
12310-1 Materials are not expected to change or react during
the period of use. Tyvek® is intended to be installed on
the cold side of the insulation and is designed to
Performance data of the product in accordance with withstand substantial temperature changes during
the declaration of performance with respect to its service life.
essential characteristics according to EN 13859-
1:2010 Flexible sheets for waterproofing - Definitions 2.11 Environment and health during use
and characteristics of underlays - Part 1: Underlays for Tyvek® membranes are usually concealed below roof
discontinuous roofing and EN 13859-2:2010 Flexible decking or facade cladding. They do not require
sheets for waterproofing - Definitions and maintenance and will not produce emissions. There
characteristics of underlays - Part 2 Underlays for walls are no environmental or health concerns to be
expected from the use of the material.
2.4 Delivery status
The single selling unit is a roll of up to 3 m width and a 2.12 Reference service life
length of up to 100 m. Usually several rolls are The documentation of the RSL is not required for this
strapped and piled on a wooden pallet. EPD since not the entire life cycle is declared (without
The order unit is square meter [m²]. modules B1-B7). Nevertheless, the product is
assumed to have a reference service life of 30 years,
2.5 Base materials/Ancillary materials corresponding to the average roof lifetime BNB
Tyvek® single layer membranes are made of Nutzungsdauerliste). But this assumption could not be
- high density polyethylene (HDPE) >99 % verified because the Tyvek® envelopes have only
- hindered amine light stabilizers (HALS, added for UV been sold for 25 years.
stabilization) <1 %.
2.6 Manufacture 2.13 Extraordinary effects
Tyvek® underlays are produced on semi-continuously
operating production facilities in different countries. Fire
Process steps include:
1. Spinning of thin HDPE filaments.
2. Bonding of filament sheet. Fire protection
3. Printing, slitting and packaging of the finished roll Name Value
goods. Building material class acc. to E on mineral wool and
EN13501-1 wood
2.7 Environment and health during
manufacturing Water
Some of the manufacturing facilities employed in the Tyvek® membranes are inherently waterproof. No part
production of Tyvek® are ISO 14001 certified. All of the product will dissolve in water nor will the product
facilities comply with local regulations and /DuPont release any toxic substances to water.
internal standards.
Particular care is taken to ensure the safety of anyone Mechanical destruction
involved in the Tyvek® supply chain in line with the No possible impacts on the environment following
DuPont safety culture: all injuries can be prevented unforeseeable mechanical destruction are known.
(goal is ZERO).
2.14 Re-use phase
2.8 Product processing/Installation The material is not intended to be re-used or recycled.
Tyvek® membranes for walls and roofs can be either Energy recovery is possible.
installed on the construction site or in manufacturing
facilities in case of pre-fabricated buildings. In both 2.15 Disposal
instances the material is usually installed by manually Disposal of the material should be made according to
unwinding the sheet from the roll and placing it onto national legislation. Incineration is the preferred way of
the designated surface. Tools required are usually a disposal. European Waste Codes (Commission
knife or scissors to cut the sheet as well as a stapler to decision 2014/955/EU) for mixed construction and
fix it to the construction. Refer to Tyvek® installation demolition waste is 17 09 04.
guidelines for more information.
2.9 Packaging 2.16 Further information
Tyvek® is wound onto carton cores. Each roll comes Additional information about product properties and
with a paper insert sheet. Rolls are individually use can be found at www.building.dupont.com.Safety
wrapped in foil (LDPE: low density PE) and stacked on Data Sheets (SDS) or Article Information Sheets (AIS)
wooden pallets which are also wrapped in LDPE of the products can be found at www.dupont.com.
3 Environmental Product Declaration DuPont de Nemours (Luxembourg) s.à r.l. – Tyvek® Monolayer 80 (1580B, 2480B)
3. LCA: Calculation rules
3.1 Declared Unit 3.6 Data quality
This declaration applies to 1 m2 of DuPont™ Tyvek® To simulate the product stage, data recorded by
1580B and 2480B membranes, with a declared unit DuPont Luxembourg s.à r.l. and the converting plant in
weight of 81 g/m2. Germany from the production year 2019 were used.
Eurostat data for the years 2018-2019 were used to
Declared Unit model the modules A4 (freight transport modal split)
Name Value Unit and A5 (packaging disposal routes).
Declared unit 1 m2 Regarding background processes, the Luxembourg
Grammage 0.081 kg/m2 and German electricity grid mix were applied to the
production plants in these countries (A1-A3). Other
background data were specific to Germany or the
European average, and were not older than 10 years.
3.2 System boundary The representativeness can be classified as very good
Type of EPD: Cradle-to-gate (with options) for all the foreground data, and most of the background
The system boundaries of the EPD follow the modular data.
construction system as described by /EN 15804:2012/.
The LCA takes into account the following modules: 3.7 Period under review
 A1-A3: Manufacturing of pre-products, The period of study encompasses the year 2019.
packaging, ancillary materials, transport to the
3.8 Allocation
factory, production including energy supply
Mass allocation was applied for production. At the
and waste handling
DuPont site in Luxembourg, Tyvek® waste materials
 A4: Transport to the construction site are sold and transformed externally. The further use of
 A5: Installation into the building (disposal of the valorized HDPE granulates was cut-off from the
packaging) system boundaries, as for the packaging materials
sent for recycling. The Tyvek® final waste material
 C4: Waste disposal (incineration)
sent to incineration is modelled through the
 D: Potential for reuse, recovery and/or
combustion process of the specific material and the
recycling (benefits for incineration and avoided conventional energy production is considered
recovery of packaging materials from module in module D. The potential benefit in module D will be
A5 and envelopes incineration from module possible only if the Tyvek® will be separate and
C4). incinerated.
3.9 Comparability
Basically, a comparison or an evaluation of EPD data
3.3 Estimates and assumptions
is only possible if all the data sets to be compared
The colour paste used in the finishing process was
were created according to EN 15804 and the building
valued with a general composition of water-based
context, respectively the product-specific
colour paste (conservative approach).
characteristics of performance, are taken into account.
3.4 Cut-off criteria
GaBi 10.5.0.78 was used to model background data.
All data were taken into consideration (recipe
constituents, process water, electricity used). In case
of missing data, a cut-off criteria of 1 % of the total
input mass was applied for unit processes and 5 % for
the
entire modules (as recommended by EN 15804,
section 6.3.5) and therefore some inputs were
excluded: tape and spiking agent for monolayer
production (sum < 0.04 % of total input mass for
monolayer production), paper ink, hotmelt, paper, tape
and detergent for finishing process (sum < 0.2 % of
total input mass for finishing process). Transports were
considered for all inputs and outputs. Manufacturing of
the production machines and systems and associated
infrastructure were not taken into account in the life
cycle assessment (LCA). Regarding possible off-cuts
during installation, the amount is lower than 5 % and
therefore also neglected.
3.5 Background data
All background data for the LCA model were taken
from the database of GaBi 10.5.0.78.
4 Environmental Product Declaration DuPont de Nemours (Luxembourg) s.à r.l. – Tyvek® Monolayer 80 (1580B, 2480B)
4. LCA: Scenarios and additional technical information
Characteristic product properties
Information on biogenic Carbon
The product does not contain biogenic carbon.
Information on describing the biogenic Carbon
Content at factory gate
Name Value Unit
Biogenic Carbon Content in
0 kg C
product
Biogenic Carbon Content in
0.0037 kg C
accompanying packaging
The following technical information serves as a basis
for the declared modules or can be used for the
development of specific scenarios in the context of a
building assessment.
Transport from the gate to the construction site
(A4)
Name Value Unit
Transport distance (weighted
3064 km
average)
Transport (train) 2.03E-02 tkm
Transport (road) 8.81E-02 tkm
Transport (water) 1.64E-01 tkm
Installation of the product into the building (A5)
Name Value Unit
Wood waste to landfill 2.97E-04 kg
Wood waste to incineration 1.78E-04 kg
Cardboard waste to landfill 2.96E-04 kg
Cardboard waste to incineration 2.26E-04 kg
Plastic waste to landfill 2.66E-05 kg
Plastic waste to incineration 3.63E-05 kg
End-of-life stage (C1-C4)
Name Value Unit
Collected separately Tyvek®
0.081 kg
waste
Energy recovery 100 %
R+ value < 0.6
5 Environmental Product Declaration DuPont de Nemours (Luxembourg) s.à r.l. – Tyvek® Monolayer 80 (1580B, 2480B)
5. LCA: Results
The results displayed below apply to 1 m2 of DuPont™ Tyvek® 1580B and 2480B membranes, with a declared
unit weight of 81 g/m2.
Disclaimers:
Potential Human exposure efficiency relative to U235: This impact category deals mainly with the eventual impact
of low dose ionizing radiation on human health of the nuclear fuel cycle. It does not consider effects due to
possible nuclear accidents, occupational exposure nor due to radioactive waste disposal in underground facilities.
Potential ionizing radiation from the soil, from radon and from some construction materials is also not measured
by this indicator.
Abiotic depletion potential for non-fossil resources; Abiotic depletion potential for fossil resources; Water (user)
deprivation potential, deprivation-weighted water consumption: The results of these environmental impact
indicators shall be used with care as the uncertainties on these results are high or as there is limited experienced
with the indicator.
Disclaimer:
EP-freshwater: This indicator has been calculated as “kg P eq” as required in the characterization model
(EUTREND model, Struijs et al., 2009b, as implemented in ReCiPe;
http://eplca.jrc.ec.europa.eu/LCDN/developerEF.xhtml).
DESCRIPTION OF THE SYSTEM BOUNDARY (X = INCLUDED IN LCA; ND = MODULE OR INDICATOR NOT
DECLARED; MNR = MODULE NOT RELEVANT)
BENEFITS AND
CONSTRUCTI LOADS
PRODUCT STAGE ON PROCESS USE STAGE END OF LIFE STAGE BEYOND THE
STAGE SYSTEM
BOUNDARIES
6 Environmental Product Declaration DuPont de Nemours (Luxembourg) s.à r.l. – Tyvek® Monolayer 80 (1580B, 2480B)
lairetam
waR
ylppus tropsnarT
gnirutcafunaM
eht
morf
tropsnarT
etis
eht
ot
etag
ylbmessA esU
ecnanetniaM
riapeR
tnemecalpeR tnemhsibrufeR
ygrene
lanoitarepO esu
retaw
lanoitarepO esu
noitcurtsnoc-eD
noitilomed tropsnarT
gnissecorp
etsaW
lasopsiD -esueR -yrevoceR -gnilcyceR laitnetop
A1 A2 A3 A4 A5 B1 B2 B3 B4 B5 B6 B7 C1 C2 C3 C4 D
X X X X X ND ND MNR MNR MNR ND ND ND ND ND X X
RESULTS OF THE LCA - ENVIRONMENTAL IMPACT according to EN 15804+A2: 1 m2 DuPont™ Tyvek®
Monolayer 80 (1580B and 2480B)
Core Indicator Unit A1-A3 A4 A5 C4 D
Global warming potential - total [kg CO2-Eq.] 3.85E-1 8.29E-3 1.85E-3 2.54E-1 -1.34E-1
Global warming potential - fossil fuels [kg CO2-Eq.] 3.85E-1 8.12E-3 1.50E-4 2.54E-1 -1.34E-1
Global warming potential - biogenic [kg CO2-Eq.] 5.60E-4 1.13E-4 1.70E-3 8.43E-6 -6.28E-4
GWP from land use and land use change [kg CO2-Eq.] 2.85E-4 5.51E-5 4.91E-8 1.36E-6 -8.43E-5
Depletion potential of the stratospheric ozone layer [kg CFC11-Eq.] 4.32E-12 6.55E-18 2.39E-19 1.90E-17 -1.38E-15
Acidification potential, accumulated exceedance [mol H+-Eq.] 1.49E-3 9.05E-5 3.89E-7 2.53E-5 -1.65E-4
Eutrophication, fraction of nutrients reaching freshwater
[kg P-Eq.] 5.86E-7 2.08E-8 3.68E-9 2.54E-9 -1.59E-7
end compartment
Eutrophication, fraction of nutrients reaching marine end
[kg N-Eq.] 2.38E-4 3.29E-5 1.70E-7 5.31E-6 -4.81E-5
compartment
Eutrophication, accumulated exceedance [mol N-Eq.] 2.56E-3 3.62E-4 1.58E-6 1.19E-4 -5.17E-4
Formation potential of tropospheric ozone photochemical
[kg NMVOC-Eq.] 8.44E-4 7.43E-5 6.85E-7 1.58E-5 -1.36E-4
oxidants
Abiotic depletion potential for non-fossil resources [kg Sb-Eq.] 5.88E-8 6.18E-10 5.04E-12 2.87E-10 -2.07E-8
Abiotic depletion potential for fossil resources [MJ] 9.67E+0 1.10E-1 8.54E-4 3.10E-2 -2.31E+0
Water (user) deprivation potential, deprivation-weighted [m³ world-Eq
3.44E-2 9.74E-5 8.61E-5 2.34E-2 -9.15E-3
water consumption (WDP) deprived]
RESULTS OF THE LCA - INDICATORS TO DESCRIBE RESOURCE USE according to EN 15804+A2: 1 m2
DuPont™ Tyvek® Monolayer 80 (1580B and 2480B)
Indicator Unit A1-A3 A4 A5 C4 D
Renewable primary energy as energy carrier [MJ] 8.57E-1 6.92E-3 8.75E-5 6.13E-3 -4.74E-1
Renewable primary energy resources as material utilization [MJ] 3.57E-4 -1.29E-14 -1.22E-16 2.55E-14 -9.57E-13
Total use of renewable primary energy resources [MJ] 8.58E-1 6.92E-3 8.75E-5 6.13E-3 -4.74E-1
Non-renewable primary energy as energy carrier [MJ] 9.67E+0 1.10E-1 8.54E-4 3.10E-2 -2.31E+0
Non-renewable primary energy as material utilization [MJ] 2.12E-4 3.53E-6 1.67E-8 1.09E-6 -7.49E-5
Total use of non-renewable primary energy resources [MJ] 9.67E+0 1.10E-1 8.54E-4 3.10E-2 -2.31E+0
Use of secondary material [kg] 3.66E-3 0.00E+0 0.00E+0 0.00E+0 0.00E+0
Use of renewable secondary fuels [MJ] 5.65E-8 0.00E+0 0.00E+0 0.00E+0 0.00E+0
Use of non-renewable secondary fuels [MJ] 6.23E-7 0.00E+0 0.00E+0 0.00E+0 0.00E+0
Use of net fresh water [m³] 4.38E-3 7.63E-6 2.05E-6 5.48E-4 -4.62E-4
RESULTS OF THE LCA – WASTE CATEGORIES AND OUTPUT FLOWS according to EN 15804+A2:
1 m2 DuPont™ Tyvek® Monolayer 80 (1580B and 2480B)
Indicator Unit A1-A3 A4 A5 C4 D
Hazardous waste disposed [kg] 1.92E-9 5.71E-12 1.54E-13 5.53E-12 -5.12E-10
Non-hazardous waste disposed [kg] 3.63E-3 1.78E-5 4.46E-4 1.01E-3 -1.01E-3
Radioactive waste disposed [kg] 1.66E-4 7.41E-7 1.79E-8 1.76E-6 -1.52E-4
Components for re-use [kg] 0.00 0.00 0.00 0.00 0.00
Materials for recycling [kg] 0.00 0.00 0.00 0.00 0.00
Materials for energy recovery [kg] 0.00 0.00 0.00 0.00 0.00
Exported electrical energy [MJ] 0.00E+0 0.00E+0 1.46E-3 5.41E-1 0.00E+0
Exported thermal energy [MJ] 0.00E+0 0.00E+0 2.08E-3 9.62E-1 0.00E+0
RESULTS OF THE LCA – additional impact categories according to EN 15804+A2-optional:
1 m2 DuPont™ Tyvek® Monolayer 80 (1580B and 2480B)
Indicator Unit A1-A3 A4 A5 C4 D
Potential incidence of disease due to PM emissions [Disease
ND ND ND ND ND
Incidence]
Potential Human exposure efficiency relative to U235 [kBq U235-
ND ND ND ND ND
Eq.]
Potential comparative toxic unit for ecosystems [CTUe] ND ND ND ND ND
Potential comparative toxic unit for humans - cancerogenic [CTUh] ND ND ND ND ND
Potential comparative toxic unit for humans - not cancerogenic [CTUh] ND ND ND ND ND
Potential soil quality index [-] ND ND ND ND ND
7 Environmental Product Declaration DuPont de Nemours (Luxembourg) s.à r.l. – Tyvek® Monolayer 80 (1580B, 2480B)
6. LCA: Interpretation
The following chart shows the relative contributions of
the different modules to the various LCA categories in
a dominance analysis.
Glossary:
For most of the impact categories, more than 70 % of
the impacts are dominated by the Tyvek® production ADPE: Abiotic depletion potential for non-fossil
(A1-A3) and in particular by the supply of HDPE resources
granulates, steam and electricity. ADPF: Abiotic depletion potential for fossil resources
The production phase represents 59 % of GWP, which AP: Acidification potential, accumulated exceedance
is also highly influenced by the final disposal (39 % of FEP: Eutrophication, fraction of nutrients reaching
the generated impact). This is due to the emissions of freshwater end compartment
carbon dioxide from the incineration plant. Fin.: Finishing process
The avoided energy production thanks to waste GWP: Global Warming Potential
incineration leads to significant benefits, which are HDPE: High-Density Polyethylene
mostly around 20 % of the impact results. LCA: Life Cycle Assessment
Waste incineration during the finishing step, including MEP: Eutrophication, fraction of nutrients reaching
Tyvek® and packaging materials, is completely marine end compartment
dominating the ODP score due to halogens emissions Mono: Monolayer production
to air in the module „EU-28: Waste incineration of Nat. gas: Natural gas
plastics (PE, PP, PS, PB)“. The transport of Tyvek® ODP: Depletion potential of the stratospheric ozone
products to the customers contributes to 12 % of MEP layer
and TEP due to the emissions of nitrogen monoxide POCP: Formation potential of tropospheric ozone
during lorry and sea transport (module A4). As photochemical oxidants
expected, the use of water, in particular cold water for TEP: Eutrophication, accumulated exceedance
monolayer production, dominates the WDP score. WDP: Water (user) deprivation potential, deprivation-
weighted water consumption
7. Requisite evidence
No requisite evidence is required for DuPont™
Tyvek® 1580B and 2480B monolayer membranes.
8 Environmental Product Declaration DuPont de Nemours (Luxembourg) s.à r.l. – Tyvek® Monolayer 80 (1580B, 2480B)
8. References
EN 12310-1
EN 12310-1:1999, Flexible sheets for waterproofing - ISO 14025
Part 1: Bitumen sheets for roof waterproofing; DIN EN ISO 14025:2011-10, Environmental labels and
determination of resistance to tearing (nail shank) declarations — Type III environmental declarations —
Principles and procedures.
EN 12311-1
EN 12311-1:1999, Flexible sheets for waterproofing - PCR, Part A
Part 1: Bitumen sheets for roof waterproofing; PCR 2021, Part A - PCR Guidance-Calculation Rules
Determination of tensile properties for the Life Cycle Assessment and Requirements on
the Project Report according to EN 15804+A2:2019
EN 1297 (version 1.1.1, 2021)
EN 1297:2004, Flexible sheets for waterproofing -
Bitumen, plastic and rubber sheets for roof PCR, Part B
waterproofing - Method of artificial ageing by long term PCR 2017, Part B - PCR Guidance-Texts for Building-
exposure to the combination of UV radiation, elevated Related Products and Services: Requirements on the
temperature and water EPD for False ceiling and underlay sheeting (version
1.6, 2017)
EN 13501-1
EN 13501-1:2007+A1:2010, Fire classification of IBU 2016
construction products and building elements - Part 1: Institut Bauen und Umwelt e.V.: General Programme
Classification using data from reaction to fire tests Instructions for the Preparation of EPDs at the Institut
Bauen und Umwelt e.V. Version 1., Berlin: Institut
EN 13859-1 Bauen und Umwelt e.V., 2016. www.ibu-epd.com
EN 13859-1:2010, Flexible sheets for waterproofing -
Definitions and characteristics of underlays - Part 1: BNB Nutzungsdauerliste
Underlays for discontinuous roofing BNB Nutzungsdauerliste: 2017. Nutzungsdaueren von
Bauteilen published by Informationsportal Nachhaltiges
EN 13859-2 Bauen des Bundesministeriums des Inneren für Bau
EN 13859-2:2010, Flexible sheets for waterproofing - und Heimat.
Definitions and characteristics of underlays - Part 2:
Underlays for walls European Waste Code
European Waste Code:2000. European List of Waste
EN 15804 European Waste Codes: (Commission decision
EN 15804:2019+A2, Sustainability of construction 2014/955/EU)
works — Environmental Product Declarations — Core
rules for the product category of construction products. Eurostat
Eurostat:2021, Data browser, Packaging waste by
EN 1848-2 waste management operations; Recycling rate of
EN 1848-2:2001, Flexible sheets for waterproofing - packaging waste by type of packaging
Determination of length, width, straightness and
flatness - Part 2: Plastic and rubber sheets for roof GaBi 10.5.0.78
waterproofing GaBi 10.5.0.78:2021. Life Cycle Engineering software
and database. Sphera Solutions GmbH, 2021.
EN 1849-2
EN 1849-2:2019, Flexible sheets for waterproofing - Regulation (EU) No. 305/2011
Determination of thickness and mass per unit area - Regulation (EU) No. 305/2011 of the European
Part 2: Plastic and rubber sheets Parliament and of the Council of 9 March 2011 laying
down harmonised conditions for the marketing of
EN 1928 construction products and repealing Council Directive
EN 1928:2000, Flexible sheets for waterproofing - 89/106/EEC
Bitumen, plastic and rubber sheets for roof
waterproofing - Determination of watertightness DuPont™, the DuPont Oval Logo, and
all trademarks and service marks denoted with ™,
EN ISO 12572 SM or ® are owned by affiliates of DuPont de
EN ISO 12572:2017, Hygrothermal performance of Nemours, Inc. unless otherwise noted.
building materials and products -- Determination of
water vapour transmission properties
EN ISO 14001
EN ISO 14001:2015, Environmental management
systems - Requirements with guidance for use (ISO
14001:2015)
9 Environmental Product Declaration DuPont de Nemours (Luxembourg) s.à r.l. – Tyvek® Monolayer 80 (1580B, 2480B)
Publisher
Institut Bauen und Umwelt e.V. Tel +49 (0)30 3087748- 0
Panoramastr. 1 Fax +49 (0)30 3087748- 29
10178 Berlin Mail info@ibu-epd.com
Germany Web www.ibu-epd.com
Programme holder
Institut Bauen und Umwelt e.V. Tel +49 (0)30 - 3087748- 0
Panoramastr 1 Fax +49 (0)30 – 3087748 - 29
10178 Berlin Mail info@ibu-epd.com
Germany Web www.ibu-epd.com
Author of the Life Cycle
Assessment Tel 00352-275888-1
Luxembourg Institute of Science Fax 00352-275888-555
and Technology (LIST) Mail info@list.lu
Avenue des Hauts-Fourneaux 5 Web www.list.lu
4362 Esch/Alzette
Luxembourg
Owner of the Declaration
DuPont de Nemours (Luxembourg) Tel +352 3666 5210
s.à r.l. Fax +352 3666 0000
Rue Général Patton 1 Mail tyvek.info@dupont.com
2984 Contern Web www.dupont.com
Luxembourg
