ENVIRONMENTAL PRODUCT DECLARATION
as per ISO 14025 and EN 15804+A2
Owner of the Declaration UAC Berhad
Publisher Institut Bauen und Umwelt e.V. (IBU)
Programme holder Institut Bauen und Umwelt e.V. (IBU)
Declaration number EPD-UAC-20240059-IBC3-EN
Issue date 05.06.2024
Valid to 04.06.2029
UAC Fiber Cement Board
UAC Berhad
www.ibu-epd.com | https://epd-online.com
1. General Information
UAC Berhad UAC Fiber Cement Board
Programme holder Owner of the declaration
IBU – Institut Bauen und Umwelt e.V. UAC Berhad
Hegelplatz 1 Jalan Portland, Tasek Industrial Estate 36
10117 Berlin 31400 Ipoh, Perak
Germany Malaysia
Declaration number Declared product / declared unit
EPD-UAC-20240059-IBC3-EN 1 tonne of UAC Fibre Cement Board
This declaration is based on the product category rules: Scope:
Fibre cement / Fibre concrete, 01.08.2021 This EPD declaration is based on the average of one metric tonne UAC
(PCR checked and approved by the SVR) Fibre Cement Board manufactured by UAC Berhad. These products are
produced in the manufacturing plant located in Ipoh, Perak (Malaysia)
where the production data for 2022 was recorded. Life Cycle Assessment
Issue date (LCA) was conducted based on the cradle-to-grave with option approach
(Modules A1-A3, A5, C1-C4 & D). The Declaration holder is liable for the
05.06.2024
details and documentation upon which the evaluation is based.
The owner of the declaration shall be liable for the underlying information
and evidence; the IBU shall not be liable with respect to manufacturer
Valid to
information, life cycle assessment data and evidences.
04.06.2029
The EPD was created according to the specifications of EN 15804+A2. In
the following, the standard will be simplified as EN 15804.
Verification
The standard EN 15804 serves as the core PCR
Independent verification of the declaration and data according to ISO
14025:2011
internally X externally
Dipl.-Ing. Hans Peters
(Chairman of Institut Bauen und Umwelt e.V.)
Florian Pronold Dr. Matthew Fishwick,
(Managing Director Institut Bauen und Umwelt e.V.) (Independent verifier)
1 Environmental Product Declaration - UAC Berhad - UAC Fiber Cement Board
2. Product
frequency from 1255000Hz. Airborne noise insulation is
2.1 Product description/Product definition determined as STC30 (tested in accordance with ASTM E90-
This is an average EPD comprises the products listed below. 09).
These autoclaved composite materials are made from specially
treated high-grade cellulose fibre, Portland cement, refined The difference between the sound absorption of the room with
sand and water. The asbestos was analyzed with a third-party and without the 6mm fibre cement
laboratory and was not found in the product. sheet is determined to obtain the total sound loss by using the
reverberation time values. Noise reduction coefficient is
The declared products include: determined as NRC0.10 (ASTM E423-90a). Sound
transmission loss (UAC Vistabord): Estimated 25dB (6mm),
- UAC Superflex/Multipurpose/Every 28dB (9mm).
- UAC Vistaboard/Flexaboard/Multiflex/Square Flex
Constructional data
- UAC Lattice (Square, Diamond)
- UAC Decoceil (Chemerah,Chemerah Plus, Tika, Angkasa, Name Value Unit
Forra, Forra Plus) Gross density 1400 kg/m3
- UAC Plank (Sedartex Woodgrain, Smooth) Standard panel thickness 6 mm
- UAC Plank Shiplap
Thermal conductivity 0.12 W/(mK)
- UAC Supertex Panel
Average Modulus of Rupture
- UAC Decowood (Woodlike, Smooth) >10 N/mm2
(saturated)
- UAC Fence
- UAC Skirting Average Modulus of Elasticity 4000 – 7000 N/mm2
- UAC Duravent (Saturated)
Moisture movement 0.06 to 0.08%
All the declared products are produced at the same process Category
Durability Classification EN12467:2012
flow with the same raw material composition with difference of A
formulation and geometrical output. For the placing on the
Strength classification EN12467:2012 Class 2
market in the Europian Union/Eueopean Free Trade
Association (EU/EFTA) (with the exception of Switzerland) the .
Regulation (EU) No. 305/2011 (CPR) applies. The product
2.4 Delivery status
needs a Declaration of Performance taking into consideration/
UAC Fibre Cement Boards are manufactured in a range of
EN 12467: 2012 Fibre cement flat sheets - product specification
thicknesses from 3.2mm to 25mm. The boards can be up to
and test methods/ and the CE- marking.
3660mm in length and up to 1220mm wide.
2.2 Application
2.5 Base materials/Ancillary materials
For the application and use the respective national provisions
The base materials, auxiliary substances and additives for UAC
apply.
Fibre Cement Boards are:
UAC Berhad manufactures a wide range of Fibre Cement
Boards which are extensively used in residential, institutional,
commercial and industrial buildings, as: -
- Internal Lining and Wall Partitioning
- Ceiling
- Soffit and Eave Lining
- Substrate for flooring
- Fire and insulation application
- Decorative application
- Roofing
- Others
2.3 Technical Data
The technical data given by the Declaration of Performance
according to EN 12467 apply.
UAC Fibre Cement Boards conform and certify to (a)
Products do not contain any substances that can be included in
MS1296:2010 for UAC Superflex and (b) EN12467:2004 for
'Candidate List of Substances of Very High Concern for
7.5mm UAC Sedartex Woodgrain Plank.
Authorization' and raw materials used are not part of the EU
REACH regulation.
Product specification
UAC Fibre Cement Board (6mm thickness) 2.6 Manufacture
- Thermal conductivity (W/mK): 0.12
Process flow of UAC Fibre Cement Board production:
- Resistance of heat transmission, Ra (m2K / W): 0.19
- Dry density (kg/m3): 1400
Soundproof:
With a 6mm fibre cement sheet (1190mmx1190mm) installed in
the opening between two adjacent but acoustically isolated
reverberation rooms, 17-33dB sound transmission loss at
2 Environmental Product Declaration - UAC Berhad - UAC Fiber Cement Board
protection analyses and close monitoring on exposure limits
have been established in accordance to the Factory and
Machineries Act (Noise Exposure) Regulations 1989 Act 139.
Waste:
All scraps and rejected UAC Fibre Cement Boards are
classified as solid waste under the Malaysia Department of
Environment (DOE) Regulations and will be treated in landfill
Act 672.
2.8 Product processing/Installation
UAC Fibre Cement Boards are cut using a guillotine knife or
circular saw with tungsten carbide, and a diamond saw blade.
Dust generated from the processes is collected through the
effective dust collecting system and filtered before release to
the air in accordance to the Factories and Machinery Act
(Mineral Dust) Regulations 1989 Act 139. Dust emission is
below the Permissible Level under Regulation 25 of the
Malaysia Environmental Quality (Clean Air) Regulations 1978
Act 127.
UAC Fibre Cement Boards are produced with the Hatschek
process or wet process: The raw materials are mixed 2.9 Packaging
homogeneously and pumped to the tubs at a controlled rate so
that tubs are filled and overflow. A uniform film is formed onto
UAC Fibre Cement Boards are packed horizontally on wooden
the sieves and the film will be picked up by felt which will then
pallets and packaged with polyethylene stretch film, PET strap
be transferred to a size roller to be rolled in layers for the
and cardboard edge protector. The wooden pallets are reused
manufacturing of a `green sheet` (intermediate product formed
internally.
during the production and yet to send to autoclave) according
to the desired thicknesses. The speed of the felt is controlled in 2.10 Condition of use
order to achieve consistent sheet thickness at a specified UAC Fibre Cement Boards have passed organic emissions
production rate. tests under the TUV Singapore emission standards for
formaldehyde, phenyl cyclohexene, phthalate, and total
Individual size roller determines the length of sheet being particles. Due to the stable crystalline calcium silicate hydrate
produced. If a patterned sheet is to be produced, a patterned phase after the autoclave process, the emission of volatile
sleeve will be placed on the size roller to create the desired organic compound (VOC) detected are low and negligible for
patterns. normal use in line with the designated purpose of the
respective products.
Once the desired thickness is achieved, it will then be
separated and taken off from the size roller by a cut-off wire. 2.11 Environment and health during use
Environmental
The green sheet will then be trimmed into size by a high- aspects: Hazards to water, soil and air cannot arise from fibre
pressure water jet while the remaining scraps will return to the cement flat sheets based on current knowledge.
scrap agitator which will then be transferred back to the feed
agitator for reuse in order to minimize generated waste. 2.12 Reference service life
The reference service life is not relevant for consideration of the
The trimmed green sheets are stacked in tiers on steel base LCA. As construction products with many different applications,
pallets. a reference service life for Fibre Cement Boards is not declared
here.
The stacked green sheets will then be air-cured for a minimum Description of the influences on the ageing of the product when
6-8 hours before curing in the autoclave for a total process applied in accordance with the rules of technology.
duration of 10-12 hours.
2.13 Extraordinary effects
The autoclaved sheets will undergo further cutting or trimming
into the final dimension at sheet finishing with either a guillotine Fire
knife or a rotating saw. Sanding, edge recessing and slotting For UAC Superflex, UAC Vistabord, UAC Decoceil, and UAC
are also being done at sheet finishing. Supertex Woodgrain panel:
Quality Management Systems in accordance to ISO 9001:2015
for design and manufacture of fibre cement products are - Fire Propagation Index: range from 0,0-3,3, according to BS
complied with. 476-6:1989.
2.7 Environment and health during manufacturing - Surface spread of flame test: Class 1 surface spread of
The UAC Berhad operation is in compliance with ISO fame (actual result 0mm at 1.5m), according to BS 476-7:1997.
45001:2018 (Occupational health and safety management
Fire protection
system).
Name Value
Water: Water
contamination was not reported during the production of UAC Building material class A2
Fibre Cement Boards. All the waste water is treated at a Burning droplets d0
designated waste water treatment plant before discharging into Smoke gas development s1
the public sewerage, in accordance to the Environmental
Quality Act 1974 Act 127.
Water
Noise: Sound
3 Environmental Product Declaration - UAC Berhad - UAC Fiber Cement Board
No substances are washed out from UAC fibre cement board
products which could be hazardous to water. 2.15 Disposal
According to Malaysia Solid Waste and Public Cleansing
Mechanical destruction Management Act 2007 Act 672, remains of UAC fibre cement
Irrelevant board waste products from construction sites or from demolition
can be disposed of as solid waste. Waste code '17 01 01
2.14 Re-use phase (Concrete)' in line with the European Waste Catalogue EWC.
Products are not designed for re-use, recycling, and recovery
(energy or otherwise), as they may impact the quality and 2.16 Further information
render unfit for their intended use. Further information on the products can be obtained from our
website www.uac.com.my
3. LCA: Calculation rules
No other estimations or assumptions were made regarding the
3.1 Declared Unit specifications outlined in this section (Chapter 3).
All products show similar recipes with some differences in the 3.4 Cut-off criteria
dosage of pre-products for certain products. Declared unit to All operating data, i.e. all of the starting materials used, internal
the UAC Fibre Cement Boards which are manufactured with the fuel consumption and electricity consumption, all direct
mixing of cement, silica sand, pulp, alumina, silica fume and red production waste as well as all emission measurements
oxide and dried under pressure and temperature in the available were taken into consideration in the analysis.
autoclave machine. Accordingly, material flows with a share of less than 1 % were
Construction materials' purpose, fixing and installation guides also considered in this study. It can be assumed that the total of
are being observed and no health impairment is known due to all neglected processes does not exceed 5 % in the effective
the basic materials employed and their behaviour according to categories. Machinery, plants and infrastructure required in the
current knowledge. manufacturing process are not taken into consideration.
Further information on the products can be referred to the
'Product Specifications' from www.uac.com.my 3.5 Background data
The average metric tonne of fibre cement products is calculated Secondary data from the LCA FE Database (Formerly GaBi)
based on the annual production data. The declared unit of this were used to model the background system in the LCA model.
study is 1 metric tonne of UAC Fibre Cement Boards with an The consistent data items contained in the LCA FE database
average bulk density of 1400 kg/m³. are documented in the online Sphera documentation centre.
Foreground data describing the on-site production are The basic data in the LCA FE database was applied for energy,
integrated into the LCA FE Software model in the study. The transportation, and consumables. The LCA was primarily
LCI is assessed based on annual production data. Background developed based on the Malaysia database. Average data from
data are taken from the LCA FE Database. the other regions were incorporated where the Malaysia
database is not available.
Declared unit
Name Value Unit 3.6 Data quality
Declared unit 1 t All background data records related to the UAC operation were
Gross density 1400 kg/m3 provided by UAC Berhad as well as the LCA FE database.
Technological: All primary and secondary data are modelled to
Conversion factor to 1 kg 0.000714286 -
be specific to the technologies or technology mixes under
For IBU core EPDs (where clause 3.6 is part of the EPD): for study. Where technology-specific data are unavailable, proxy
average EPDs, an estimate of the robustness of the LCA data are used. The overall technological representativeness is
values must be made, e.g. concerning the variability of the considered to be good.
production process, geographical representativeness and the
influence of background data and preliminary products Geographical: All primary and secondary data are collected
compared to the environmental impacts caused by the actual specific to the country / region under study. Where
production. country/region-specific data are unavailable, proxy data are
used. The overall geographical representativeness is
considered to be good.
3.2 System boundary
Type of EPD: Cradle to gate with options. Temporal: All primary data are collected for a representative
year. All secondary data come from the Sphera LCA FE
The following life cycle stages were included: A1-A3, A5, C1, Databases and are representative of the years 2020-2025. As
C2, C3, C4 and D. the study for the product systems is based on the reference
year 2022, temporal representativeness is good.
Manufacture of preliminary products (cement, sand, pulp,
alumina, silica fume and red pigment) and transportation of raw 3.7 Period under review
materials and preliminary products to the plant have been The LCA study was developed based on the operation activities
considered. Manufacturing process in the plan including energy, from January to December of 2022.
manufacture of auxiliaries, disposal of residual materials
incurred and consideration of any emissions incurred. 3.8 Geographic Representativeness
Manufacture of packaging materials has also been considered. Land or region, in which the declared product system is
manufactured, used or handled at the end of the product´s
lifespan: Malaysia
3.3 Estimates and assumptions 3.9 Allocation
4 Environmental Product Declaration - UAC Berhad - UAC Fiber Cement Board
No allocation was applied in the life cycle assessment for the according to EN 15804 and the building context, respectively
foreground data of the examined products. the product-specific characteristics of performance, are taken
into account. The main LCA database used in the study is the
3.10 Comparability Sphera MLC and Sphera LCA FE CUP 2023.2.
Basically, a comparison or an evaluation of EPD data is only
possible if all the data sets to be compared were created
4. LCA: Scenarios and additional technical information
materials has been considered. The thermal and energy credit
Characteristic product properties of biogenic carbon with Malaysian dataset has been considered.
Name Value Unit
The biogenic carbon content quantifies the amount of biogenic
carbon in a construction product leaving the factory gate, and it
shall be separately declared for the product and for any In case a reference service life according to applicable ISO
accompanying packaging. standards is declared then the assumptions and in-use
conditions underlying the determined RSL shall be declared. In
addition, it shall be stated that the RSL applies to the reference
Information on describing the biogenic carbon content at
conditions only.
factory gate
Name ValueUnit The same holds for a service life declared by the manufacturer.
kg Corresponding information related to in-use conditions needs
Biogenic carbon content in product 29.49
C not be provided if a service life taken from the list of service life
Biogenic carbon content in accompanying kg by BNB is declared.
0.17
packaging C
End of life (C1-C4)
Note: 1 kg of biogenic carbon is equivalent to 44/12 kg of CO .
2
Name Value Unit
Collected separately waste type waste type 1000 kg
Landfilling 1000 kg
Installation into the building (A5) 100% landfill has been considered in the end-of-life of the
The installation (Screws, adhesives etc. along with electricity product.
consumption) phase could not be modelled due to data
unavailability. In module A5 the incineration of the packaging
5 Environmental Product Declaration - UAC Berhad - UAC Fiber Cement Board
5. LCA: Results
DESCRIPTION OF THE SYSTEM BOUNDARY (X = INCLUDED IN LCA; MND = MODULE OR INDICATOR NOT DECLARED; MNR
= MODULE NOT RELEVANT)
Benefits and
Construction loads beyond
Product stage Use stage End of life stage
process stage the system
boundaries
la ire ta m w a Ry lp p u s tro p s n a rT g n iru tc a fu n a M e h t m o rf tro p s n a rTe tis e h t o t e ta g y lb m e s s A e s U e c n a n e tn ia M ria p e R tn e m e c a lp e R tn e m h s ib ru fe R y g re n e la n o ita re p Oe s u re ta w la n o ita re p Oe s u n o itc u rts n o c -e Dn o itilo m e d tro p s n a rT g n is s e c o rp e ts a W la s o p s iD -e s u e R-y re v o c e R-g n ilc y c e Rla itn e to p
A1 A2 A3 A4 A5 B1 B2 B3 B4 B5 B6 B7 C1 C2 C3 C4 D
X X X MND X MND MND MNR MNR MNR MND MND X X X X X
RESULTS OF THE LCA - ENVIRONMENTAL IMPACT according to EN 15804+A2: 1 tonne UAC Fiber Cement Boards with
Average Bulk density 1400 kg/cum
Parameter Unit A1-A3 A5 C1 C2 C3 C4 D
GWP-total kg CO 2 eq 6.44E+02 1.98E+00 4.63E-01 3.88E+00 0 1.14E+02 -1.22E+00
GWP-fossil kg CO 2 eq 7.43E+02 1.41E+00 4.63E-01 3.3E+00 0 1.48E+01 -1.22E+00
GWP-biogenic kg CO 2 eq -1E+02 5.77E-01 1.3E-04 5.35E-01 0 9.92E+01 -2.26E-04
GWP-luluc kg CO 2 eq 3.73E-01 4.79E-06 1.21E-04 5.07E-02 0 4.67E-02 -2.16E-04
ODP kg CFC11 eq 5.23E-10 1.52E-13 3.46E-13 8.73E-14 0 3.82E-11 -6.05E-13
AP mol H+ eq 2.95E+00 2.96E-04 2.1E-03 4.56E-03 0 1.07E-01 -4.17E-03
EP-freshwater kg P eq 1.53E-03 4.12E-08 1.82E-07 3.2E-06 0 3.03E-05 -3.2E-07
EP-marine kg N eq 1.11E+00 9.02E-05 6.41E-04 1.49E-03 0 2.75E-02 -1.36E-03
EP-terrestrial mol N eq 1.2E+01 1.37E-03 7.01E-03 1.84E-02 0 3.03E-01 -1.49E-02
kg NMVOC
POCP 3.07E+00 2.47E-04 1.74E-03 3.89E-03 0 8.31E-02 -3.73E-03
eq
ADPE kg Sb eq 1.99E-05 1.41E-09 7.37E-09 8.43E-07 0 6.94E-07 -1.29E-08
ADPF MJ 7.34E+03 3.87E-01 5.21E+00 5.1E+01 0 2E+02 -1.57E+01
m3 world eq
WDP 1.03E+01 2.04E-01 3.48E-03 1.35E-02 0 1.65E+00 -6.25E-03
deprived
GWP = Global warming potential; ODP = Depletion potential of the stratospheric ozone layer; AP = Acidification potential of land and water; EP =
Eutrophication potential; POCP = Formation potential of tropospheric ozone photochemical oxidants; ADPE = Abiotic depletion potential for non-fossil
resources; ADPF = Abiotic depletion potential for fossil resources; WDP = Water (user) deprivation potential)
RESULTS OF THE LCA - INDICATORS TO DESCRIBE RESOURCE USE according to EN 15804+A2: 1 tonne UAC Fiber Cement
Boards with Average Bulk density 1400 kg/cum
Parameter Unit A1-A3 A5 C1 C2 C3 C4 D
PERE MJ 1.48E+03 7.48E+00 5.78E-01 3.27E+00 0 1.24E+03 -1.01E+00
PERM MJ 1.21E+03 -7.38E+00 0 0 0 -1.21E+03 0
PERT MJ 2.69E+03 9.64E-02 5.78E-01 3.27E+00 0 3.26E+01 -1.01E+00
PENRE MJ 7.32E+03 2.37E+01 5.21E+00 5.1E+01 0 2E+02 -1.58E+01
PENRM MJ 2.33E+01 -2.33E+01 0 0 0 0 0
PENRT MJ 7.34E+03 3.88E-01 5.21E+00 5.1E+01 0 2E+02 -1.58E+01
SM kg 0 0 0 0 0 0 0
RSF MJ 0 0 0 0 0 0 0
NRSF MJ 0 0 0 0 0 0 0
FW m3 4.72E+00 4.8E-03 1.22E-03 5.56E-03 0 5.05E-02 -2.13E-03
PERE = Use of renewable primary energy excluding renewable primary energy resources used as raw materials; PERM = Use of renewable primary
energy resources used as raw materials; PERT = Total use of renewable primary energy resources; PENRE = Use of non-renewable primary energy
excluding non-renewable primary energy resources used as raw materials; PENRM = Use of non-renewable primary energy resources used as raw
materials; PENRT = Total use of non-renewable primary energy resources; SM = Use of secondary material; RSF = Use of renewable secondary fuels;
NRSF = Use of non-renewable secondary fuels; FW = Use of net fresh water
RESULTS OF THE LCA – WASTE CATEGORIES AND OUTPUT FLOWS according to EN 15804+A2:
1 tonne UAC Fiber Cement Boards with Average Bulk density 1400 kg/cum
Parameter Unit A1-A3 A5 C1 C2 C3 C4 D
HWD kg 1.64E-05 1.02E-11 1.61E-10 1.05E-10 0 4.36E-09 -7.14E-10
NHWD kg 2.3E+02 2.4E-02 1.28E-03 2.01E-03 0 1E+03 -3.28E-03
RWD kg 4.3E-02 2.21E-05 6.62E-07 4.84E-06 0 2.28E-03 -1.49E-06
CRU kg 0 0 0 0 0 0 0
MFR kg 0 0 0 0 0 0 0
MER kg 0 9.65E-01 0 0 0 0 0
EEE MJ 0 3.47E+00 0 0 0 0 0
6 Environmental Product Declaration - UAC Berhad - UAC Fiber Cement Board
EET MJ 0 6.22E+00 0 0 0 0 0
HWD = Hazardous waste disposed; NHWD = Non-hazardous waste disposed; RWD = Radioactive waste disposed; CRU = Components for re-use;
MFR = Materials for recycling; MER = Materials for energy recovery; EEE = Exported electrical energy; EET = Exported thermal energy
RESULTS OF THE LCA – additional impact categories according to EN 15804+A2-optional:
1 tonne UAC Fiber Cement Boards with Average Bulk density 1400 kg/cum
Parameter Unit A1-A3 A5 C1 C2 C3 C4 D
Disease
PM 4.77E-05 1.65E-09 1.73E-08 3.08E-08 0 1.31E-06 -3.43E-08
incidence
IR kBq U235 eq 7.16E+00 3.55E-03 8.36E-05 4.76E-04 0 2.64E-01 -2.06E-04
ETP-fw CTUe 4.56E+03 1.54E-01 4.21E-01 9.7E+00 0 1.08E+02 -8.12E-01
HTP-c CTUh 1.36E-07 1.39E-11 5.49E-11 2.01E-10 0 1.68E-08 -1.85E-10
HTP-nc CTUh 6.34E-06 2.33E-10 7.25E-10 6.13E-09 0 1.77E-06 -1.44E-09
SQP SQP 1.51E+04 1.18E-01 3.83E-01 3.97E+01 0 4.86E+01 -6.71E-01
PM = Potential incidence of disease due to PM emissions; IR = Potential Human exposure efficiency relative to U235; ETP-fw = Potential comparative
Toxic Unit for ecosystems; HTP-c = Potential comparative Toxic Unit for humans (cancerogenic); HTP-nc = Potential comparative Toxic Unit for humans
(not cancerogenic); SQP = Potential soil quality index
Disclaimer 1 – for the indicator “Potential Human exposure efficiency relative to U235”. This impact category deals mainly with the
eventual impact of low-dose ionizing radiation on human health of the nuclear fuel cycle. It does not consider effects due to possible
nuclear accidents, occupational exposure or radioactive waste disposal in underground facilities. Potential ionizing radiation from the
soil, radon and from some construction materials is also not measured by this indicator.
Disclaimer 2 – for the indicators “abiotic depletion potential for non-fossil resources”, “abiotic depletion potential for fossil resources”,
“water (user) deprivation potential, deprivation-weighted water consumption”, “potential comparative toxic unit for ecosystems”,
“potential comparative toxic unit for humans – cancerogenic”, “Potential comparative toxic unit for humans - not cancerogenic”,
“potential soil quality index”. The results of this environmental impact indicator shall be used with care as the uncertainties on these
results are high as there is limited experience with the indicator.
6. LCA: Interpretation
In terms of environmental impacts, due to the energy- and Module A2 (7.83%).
resources-intensity of the raw material production processes,
the cement production was recorded to be the major contributor The total cradle to gate (Module A1-A3) AP is 2.95 kg H+eq. in
to the environmental indicators for the production of 1 tonne which major contribution is coming from Module A3 (40.33%)
UAC Fibre Cement Board. followed by Module A2 (30.57%) and Module A1 (29.10%).
This study revealed that the manufacturing activities within the The total cradle to gate (Module A1-A3) ADPE-element is 1.99
UAC Plant had an equivalent environmental impact profile as E-05 kg Sb-eq in which major contribution is coming from
compared to the raw material production process. Module A1 (76.49%) followed by Module A3 (16.73%).
In overall, the production (Module A1-A3) of 1 tonne of UAC The total cradle to gate (Module A1-A3) ADPE-fossil is 7340.17
Fibre Cement Board contributed 743.41 kg CO 2eq of GWP MJ in which the significant contribution is coming from Module
(Global warming potential, fossil) in which the Module A1 A1 (45.91%) and Module A3 (44.14%) followed by Module A2
contributes 55.69% and Module A3 (36.48%) followed by (9.95%).
7. Requisite evidence
7.1 Radioactivity Name Value Unit
Measurement of the nuclide content in Bq/kg for Ra-226, Th-
Arsenic (As) < 0.018 mg/L
232, K-40. In Germany, there are currently no statutory limit
Barium (Ba) ≤ 0.16 mg/L
values specified for assessing the radioactivity of building
Cadmium (Cd) ≤ 0.0013 mg/L
materials. Assessment can be performed on the basis of:
Chromium (Cr) ≤ 0.017 mg/L
- EU Commission "Radiation Protection 112" document Mercury (Hg) ≤ 0.002 mg/L
- OENORM 5200-Nordic Countries' Recommendation 2000. Plumbum (Pb) ≤ 0.02 mg/L
Testing on the toxicity characteristic leaching procedure (TCLP)
Selenium (Se) ≤ 0.02 mg/L
using SW 846 6010 and 7473 methods were conducted for
Silver (Ag) < 0.01 mg/L
UAC Fibre Cement Board (represented by Flexabord and
Superflex) where the results are demonstrated in the table The 'ASTM D5116-06: Standard Guide for small smallscale
below. environmental chamber determinations of organic emissions
from indoor materials/products' testing conducted by TUV
Singapore certified that UAC Fibre Cement Board is:
Leaching Test
VOC emissions
7 Environmental Product Declaration - UAC Berhad - UAC Fiber Cement Board
Name Value Unit * Detection level: 0.002 mg per m^3
Total VOC emission rate 0.17 mg/cum/hour
per
Formaldehyde emission <0.02
cum/hour
Phenyl cyclohexene emission Not dectecte per
rate d* cum/hour
Phthalate emission 0.003 per m3
Total particle emission <0.02 per m3
8. References
ISO 9001
Act 127 ISO 9001: 2015 -Quality management systems requirements
Laws of Malaysia Act 127 – Environmental Quality Act 1974 –
Environmental Quality (Clean Air) Regulations, 1978 ISO 14025
DIN EN ISO 14025:2011-10 Environmental labels and
Act 139 declarations — Type III environmental declarations —
Laws of Malaysia Act 139 – Factories and Machinery Act 1967 Principles and procedures
– Factories and Machinery (Mineral Dust) Regulations 1989
ISO 14040
Laws of Malaysia Act 139 – Factories and Machinery Act 1967 ISO 14040:2006: Environmental management – Lifecycle
– Factories and Machinery (Noise Exposure) Regulations 1989 assessment – Principles and framework.
Act 672 ISO 14044
Laws of Malaysia Act 672 – Solid Waste and Public Cleansing ISO 14044:2006: Environmental management – Lifecycle
Management Act 2007 assessment – Requirements and guidelines
ASTM D5116-06 LCA FE (Formerly GaBi): Software and database for life cycle
Standard Guide for small small-scale environmental chamber engineering. LBP, University of Stuttgart and thinkstep AG,
determinations of organic emissions from indoor Leinfelden-Echterdingen, 2023
materials/products
LCA FE (Formerly GaBi): Documentation of GaBi 10.6-
ASTM E90-09 Datasets for life cycle engineering. LBP University of Stuttgart
Standard Test Method for Laboratory Measurement of Airborne and thinkstep AG, 2023.
Sound Transmission Loss of Building Partitions and Elements
https://sphera.com/product-sustainability-gabi-data-search/
ASTM E 423: Standard test method for normal spectral
Method 6010 -
BS 476 Part 6. Inductively Coupled Plasma-Atomic Emission Spectrometry
Fire propagation. Source:
http://www.colorcoatonline.com/en/technical/regulations/fire_performancMeeemth/obditt a7n4c7e3 -
Mercury in Solids and Solutions by Thermal Decomposition,
BS 476 Part 7. Amalgamation, and Atomic Absorption Spectrophotometry
Surface spread of flame. Source:
http://www.colorcoatonline.com/en/technical/regulations/fire_performanMS1296
Malaysia Standard MS 1296: 2010 Fibre-Cement Flat Sheets
BS EN 12467:2004
Fibre-cement flat sheets. Product specification and test PCR 2021, Part A & B
methods Institut Bauen and Umwelt e,V, Berlin (pub): Product Category
Rules for Construction products from the range of
EN 15804 Environmental Product Declarations of Institut Bauen und
EN 15804:2012+A2:2019+AC: 2021, Sustainability of Umwelt(IBU), Part A: Calculation Rules for the Life Cycle
construction works — Environmental Product Declarations — Assessment and Requirements on the Background Report
Core rules for the product category of construction products version 1.3, 2021, Part B: Requirement on the EPD by fibre
cement/ fibre concrete, version 1.6, 01.08.2021, www.bau-
European Waste Catalogue (EWC) mwelt.de
Chapter 17: Construction and demolition wastes (including
excavated soil from contaminated sites) SW 846
Test Methods for Evaluating Solid Waste, Physical / Chemical
IBU 2016 Methods
IBU (2016): General Programme Instructions for the
Preparation of EPDs at the Institut Bauen und Umwelt e.V.,
Version 1.1 Institut Bauen und Umwelt e.V., Berlin.
8 Environmental Product Declaration - UAC Berhad - UAC Fiber Cement Board
Publisher
Institut Bauen und Umwelt e.V. +49 (0)30 3087748- 0
Hegelplatz 1 info@ibu-epd.com
10117 Berlin www.ibu-epd.com
Germany
Programme holder
Institut Bauen und Umwelt e.V. +49 (0)30 3087748- 0
Hegelplatz 1 info@ibu-epd.com
10117 Berlin www.ibu-epd.com
Germany
Author of the Life Cycle Assessment
thinkstep Sustainability Solutions Pvt. Ltd., a Sphera +91 99671 06584
company ragrawal@sphera.com
Meadows, Sahar Plaza 707 www.sphera.com
400059 Mumbai
India
Owner of the Declaration
UAC Berhad +605 – 291 2033
Jalan Portland, Tasek Industrial Estate 36 chen_lin_shiung@uac.com.my
31400 Ipoh, Perak www.uac.com.my
Malaysia
9 Environmental Product Declaration - UAC Berhad - UAC Fiber Cement Board
