ENVIRONMENTAL PRODUCT DECLARATION
as per ISO 14025 and EN 15804+A2
Owner of the Declaration Unilin B.V. Division Panels
Publisher Institut Bauen und Umwelt e.V. (IBU)
Programme holder Institut Bauen und Umwelt e.V. (IBU)
Declaration number EPD-UNI-20230380-IBJ1-EN
Issue date 31.10.2023
Valid to 30.10.2028
Unilin Decorative Compact MDF
Unilin B.V. Division Panels
www.ibu-epd.com | https://epd-online.com
1. General Information
Unilin B.V. Division Panels Unilin Decorative Compact MDF
Programme holder Owner of the declaration
IBU – Institut Bauen und Umwelt e.V. Unilin B.V. Division Panels
Hegelplatz 1 Ooigemstraat 3
10117 Berlin 8710 Wielsbeke
Germany Belgium
Declaration number Declared product / declared unit
EPD-UNI-20230380-IBJ1-EN 1 m² of Unilin decorative compact MDF board (11.15 kg/m²)
This declaration is based on the product category rules: Scope:
Wood-based panels, 01.08.2021 The scope of this EPD covers Unilin's melamine faced Fibromax Compact
(PCR checked and approved by the SVR) MR Black. This fiberboard is produced in the following manufacturing sites:
Raw board
Issue date
• Bazeilles, France
31.10.2023
Melamine faced board
• SPANO, Oostrozebeke, Belgium
Valid to • BOSPAN, Wielsbeke, Belgium
30.10.2028
The owner of the declaration shall be liable for the underlying information
and evidence; the IBU shall not be liable with respect to manufacturer
information, life cycle assessment data and evidences.
The EPD was created according to the specifications of EN 15804+A2. In
the following, the standard will be simplified as EN 15804.
Verification
The standard EN 15804 serves as the core PCR
Independent verification of the declaration and data according to ISO
14025:2011
Dipl.-Ing. Hans Peters
(Chairman of Institut Bauen und Umwelt e.V.) internally X externally
Florian Pronold Mr Olivier Muller,
(Managing Director Institut Bauen und Umwelt e.V.) (Independent verifier)
1 Environmental Product Declaration - Unilin B.V. Division Panels - Unilin Decorative Compact MDF
2. Product
2.1 Product description/Product definition 2.3 Technical Data
The Unilin decorative compact medium density fiberboard Technical characteristics vary by thickness. More detailed
(MDF) consists of a raw board that is pressed with an product-specific data, technical data sheets and the CE
impregnated paper, both on the product's front and backside. declaration of performance are available on
The decor on the panel is obtained by applying a printed decor www.unilinpanels.com.
paper on the raw board. The texture is pressed into the
Constructional and surface data
melamine surface under high pressure and high temperature
The table below summarizes the technical performance of a 10
using a special press plate technology.
mm Unilin decorative compact MDF board for some
parameters. Please check the specific "Declaration Of
The raw board is a high density moisture resistant MDF board
Performance" available on www.unilinpanels.com for additional
(> 1000 kg/m3), with a black-colored core. The surface does not
parameters or values for other thicknesses.
require further treatment and can be applied in all types of
Name Value Unit
interior projects. The decorative board is durable, scratch
resistant, colorfast and easy to maintain. More than 80 designs Grammage @ 15.9 mm
11.15 kg/m²
are available in Unilin's Decorative range (e.g. woods, plain (EN 323)
colors and materials). Bending strength (EN
58 N/mm²
310)
E-modulus (EN 310) 6000 N/mm²
For the placing on the market of the product in the European
Thermal conductivity (EN
Union/European Free Trade Association (EU/EFTA) (with the 0.13 W/(mK)
13986)
exception of Switzerland) Regulation (EU) No. 305/2011 (CPR)
Sound absorption 250 -
applies. The product needs a declaration of performance 0.10
500 HZ (EN 13986)
according:
Sound absorption 1000 -
• EN 13986:2004+A1:2015, Wood-based panels for use 0.20
2000 HZ (EN 13986)
in construction – Characteristics, valuation of conformity
E1(*); E0.5 (**);
and marking
Formaldehyde CARB/TSCA Title VI (***);
• EN 14322:2021, Wood-based panels - Melamine faced
F**** (****)
boards for interior uses - Definition, requirements and
classification Surface Soundness (EN
> 1 N/mm²
• EN 622-5:2010, Fibreboards - Specifications - Part 5: 311)
Requirements for dry process boards (MDF) Thickness tolerance (EN
± 0.2 mm
324)
For the application and use the respective national provisions
Different formaldehyde emission standards are available
apply.
(*) E1 - According to EN 13986+A1:2015 :
The results in this EPD refer to the environmental impact of a • a limit value of 0.1 ppm may not be exceeded by EN
10 mm Unilin Evola (Basic)/Customized Design Fibromax 717-1 emission chamber method OR
Compact MR Black. The declared impact is representative for • a limit value of 8 mg HCHO/100 g according to ISO
other thicknesses, although their values can vary from the 12460-5
declared ones. Please contact Unilin's sales team or
info.panels@unilin.com for more information. (**) E0.5 - According to the ChemVerbotsV :
• a limit value of 0.1 ppm according to EN 16516 OR
2.2 Application
• a limit value of 0.05 ppm according to EN 717-1
Decorative compact MDF boards are commonly used for heavy
duty surfaces thanks to the high density of the substrate. These
(***) CARB 2/TSCA Title VI - According to California Air
melamine faced fiberboards are commonly applied in interior
Resources Board & the US Toxic Substances Control Act
furniture and decorative interior design in both residential and
(TSCA Title VI) :
commercial projects. Target segments are retail, office and
• a limit value of 0.09 ppm according to ASTM E1333 or
hotel. The main applications for the melamine faced panel are
ASTM D6007
listed below:
(****) F**** - According to Japanese standard JIS A 5908
• Toilet areas
• Lockers • a limit value of 0.3 mg/L according to JIS A 1460
• Changing rooms desiccator
• Upmount sinks
• Product presentations and displays Performance data are consistent with the product's declaration
• Intensively used furniture of performance with respect to its essential characteristics
according to:
The product meets the surface specifications of a twosided HPL
• EN 13986:2004+A1:2015, Wood-based panels for use
compact board and can thus be used in similar applications
in construction – Characteristics, valuation of conformity
(with the exception of showers and undermount sinks).
and marking
• EN 14322:2021, Wood-based panels - Melamine faced
All melamine faced boards demonstrate low formaldehyde
boards for interior uses - Definition, requirements and
emissions (since the core board is coated).
classification
• EN 622-5:2010, Fibreboards - Specifications - Part 5:
Requirements for dry process boards (MDF)
2 Environmental Product Declaration - Unilin B.V. Division Panels - Unilin Decorative Compact MDF
Melamine faced board
2.4 Delivery status
1. The raw decor paper is impregnated with an
Unilin's decorative compact MDF boards are available in a
urea/melamine formaldehyde resin.
diverse range of dimensions:
2. The impregnated paper is dried, cut to the correct size
• Length: 2000 - 5600 mm and stacked on pallets or rolls.
• Width: 1220 - 2100 mm 3. The press plates, which contain the required surface
• Thickness: 6 - 13 mm finish, are placed into the melamine press facing the
front- as well as the backside of the panel. The
Please contact Unilin's sales team or info.panels@unilin.com impregnated paper is positioned on both sides of the
for more information on available dimensions. raw board.
4. The hot press closes for certain amount of time, during
2.5 Base materials/Ancillary materials
which the resin bonds the decor paper to the raw board.
The data below details the composition of a 10 mm melamine 5. The panel undergoes an additional quality check and is
faced Fibromax Compact MR Black. removed if necessary
6. After cooling down, the melamine faced board can be
Compostion raw board stacked on a pallet.
The raw MDF board has a density of 1080 kg/m³ and consists
of fresh wood, melamine urea formaldehyde (MUF) glue, 2.7 Environment and health during manufacturing
additives (e.g. wax emulsion) and moisture. Unilin's plant management policy is fully integrated in the daily
Name Value Unit operation and governance of its production plants. The aim is to
adhere to legal requirements, minimize negative environmental
Fresh wood 72 %
effects on its neighbors, co-workers and surroundings, and
Glue 19 %
constantly improve environmental performance. The Bazeilles
Additives 3 %
site is certified under ISO 9001 and ISO 50001. The BOSPAN
Moisture 6 % and SPANO plants are ISO 9001 certified.
The fresh wood is 100 % recovered wood, predominantly
The implementation of Unilin's One Home Sustainability
sourced from sustainable forest management activities and
Strategy and its Zero Harm Safety Policy have further set clear
sawmills (residues & co-products), and mainly consists of
targets to among others reduce the carbon footprint of its
spruce, beech and birch.
production activities, improve the overall resource efficiency
and enhance the safety and well-being at its production sites.
Composition decorative board (10 mm)
The decorative product has a grammage of 11.15 kg/m² and
2.8 Product processing/Installation
consists of a raw compact MDF board and 2 impregnated decor
Unilin's decorative compact MDF board can be processed (e.g.
paper layers, covering the front and back of the core board. The
sawing, milling, drilling) using common utility tools and
decor papers are impregnated with an urea/melamine
machinery. It is advised to wear a dust mask when tools are
formaldehyde resin to ensure adhesion to the surface of the
used without dust extraction. More specific processing and
raw board. This impregnated decor paper has a sales-weighted
health information is available at www.unilinpanels.com.
average grammage of 173 g/m².
2.9 Packaging
The decorative MDF board thus has the following composition:
Product packaging is used to protect the product from damage
• Raw board: 97 % during transport. Wood-based chipboards, cardboard, stretch
• Impregnated decor paper (front + back): 3 % foil and PET packaging straps are used as packaging materials.
The composition of specific thicknesses can differ from the 2.10 Condition of use
values depicted above and can be obtained by reaching out to The product's composition remains unchanged during its use
info.panels@unilin.com. and is therefore the same as stated in section 2.5. The glue,
resin and additives are permanently bonded to the wood and
Unilin's decorative fiberboard contains Substances of Very High paper through an irreversible curing process.
Concern (SVHCs) or Category 1A or 1B CMR-substances (as
2.11 Environment and health during use
defined by ECHA) above 0.1 % by weight: No
The board further contains no biocides as defined under the EU Based on current knowledge, using Unilin's decorative
Biocidal Products Ordinance No. 528/2012 nor are the boards fiberboard as intended poses no risks to health, water, air or
treated with such substances. soil. Small amounts of natural wood constituents could
potentially be released, but aside from negligible amounts of
2.6 Manufacture formaldehyde, no harmful emissions have been detected.
Raw board
2.12 Reference service life
1. Round wood is collected to produce the fiberboards.
The reference service life (RSL) of the product depends
2. The bark is removed from the round wood logs.
significantly on its field of use. Please contact Unilin's sales
3. The logs are chopped to wood chips.
team or info.panels@unilin.com for more specific information
4. The wood chips are defibrated under high pressure in a
on the product's lifespan in a given set of conditions.
refiner.
5. The board is produced by introducing the fibermat into a
The RSL of a melamine faced compact MDF board can vary
press, which compresses it under higher pressure and
from 10 to 40 years depending on its area of application;
temperature.
according to the BBSR table "BNB Nutzungsdauern von
6. The board is sanded, cut into panels and finished
Bauteilen (2017)".
depending on the intended application.
3 Environmental Product Declaration - Unilin B.V. Division Panels - Unilin Decorative Compact MDF
the Unilin decorative fiberboard can easily be abstracted and
2.13 Extraordinary effects collected if selective dismantling/sorting takes place. After
Fire collection, the end-of-life fiberboard can be reused for the same
The product has the following fire behavior (according to (or different) purpose if possible.
EN13501-1):
Energy Recovery
CE AVCP Class 4 : In line with the cascading use of wood-based products, the
• Unilin Evola (Basic)/Customized Design - Fibromax reuse of the end-of-life compact MDF should be prioritized.
Compact MR Black: D-s2,d0 (≥ 9 mm/ Bulk density > However, if this is not feasible, the board can be used as a
600 kg/m³) secondary fuel in approved energy power plants. Its relatively
high calorific value enables power plants to effectively produce
Fire reaction classes are part of the CE Declaration of renewable heat and electricity.
Performance available on Unilin Panels' website
2.15 Disposal
www.unilinpanels.com.
Jobsite and post-consumer compact MDF-waste (e.g. from
demolition projects) should be reused/recycled where possible,
in line with the cascade principle. Should this not be possible,
Water
the waste must be utilized for energy recovery as opposed to
The melamine faced board does not contain substances that
being landfilled (in accordance with EWC waste codes
may potentially contaminate water through leaching.
170201/030105).
Mechanical destruction
Waste from packaging materials, which protect the product
When subjected to mechanical stress, the product displays a
from damage during transport, can be reused and recycled if
tendency towards brittleness. This could result in the formation
sorted correctly.
of splinters and sharp broken edges, which may pose a risk of
injury.
2.16 Further information
2.14 Re-use phase Please contact Unilin's sales team or reach out to
info.panels@unilin.com for additional information.
Reuse/Recycling
When a building or furniture has reached its end-of-life phase,
3. LCA: Calculation rules
energy from these woody waste streams, which is directly
3.1 Declared Unit supplied to the SPANO and BOSPAN plants. Any remaining
The declared information and values refer to 1 m² of Unilin's energy needs are met through the local grid in Belgium or
melamine faced Fibromax Compact MR Black with a France.
grammage of 11.15 kg/m² and thickness of 10 mm.
Declared unit and mass reference C1: Deconstruction/Demolition stage
It is assumed that the end-of-life decorative fiberboard is
Name Value Unit
manually dismantled from the building/furniture. The efforts
Declared unit 1 m2 involved in this process are considered negligible, leading to
Grammage 11.15 kg/m2 the absence of a declared environmental impact arising from
Layer thickness 0.01 m the dismantling of the product.
The raw board is manufactured at the Bazeilles plant. The
C2: Transport to Waste Processing
decorative board is produced at the SPANO and BOSPAN
This life cycle stage describes the impact of the end-of-life
sites. All of these production facilities are in scope of the
product's transport from the demolition site to the waste
declaration.
processing facility. A representative distance of 50 km is
assumed.
3.2 System boundary
This is a cradle-to-gate EPD with options, including the
C3: Waste Processing
following life cycle phases A1 - A3, C1 - C4 and D. The
Processing of post-consumer compact MDF waste involves
following processes have been considered for each of the
(preliminary) sorting and shredding of the material. The
modules:
fiberboard is repurposed as a secondary fuel and undergoes
energy recovery in module D. The material and its inherent
A1 - A3: Product Stage
properties (e.g. biogenic carbon and primary energy content)
The production stage encompasses the extraction of raw
are thus exported from the system in C3.
materials (i.e. wood, paper, glue, resin, additives), their
transportation to the production plants, and the subsequent
C4: Waste Disposal
manufacturing of the product. The required energy for
This module describes the loads and emissions attributed to
production, ancillary materials, and production emissions are
the disposal of the product after waste processing. As the end-
included. Energy and material input/output data were obtained
of-life product leaves the system in C3 as a secondary fuel, no
from Unilin's Bazeilles, SPANO and BOSPAN plants as well as
environmental impact is declared in C4.
its glue factory.
D: Loads and Benefits beyond the System Boundaries
A large share of the supplied production energy consists of
Module D describes the loads and benefits related to the use of
renewable energy, derived from non-recyclable woody waste
the end-of-life compact MDF as a secondary fuel. This involves
streams. These waste streams are sourced in- and externally.
the energy recovery of post-consumer fiberboard waste, where
Unilin's fiberboard plant generates renewable thermal energy
it replaces a European-averaged mix of electricity and heat.
on-site. The biomass plants, A&S and A&U, produce renewable
4 Environmental Product Declaration - Unilin B.V. Division Panels - Unilin Decorative Compact MDF
The system boundary between subsequent systems is defined
in accordance with EN 15804+A2, i.e. when the material 3.6 Data quality
reaches its end-of-waste state. End-of-life fiberboard reaches Data collection and necessary calculations were done in line
its end-of-waste state after a sorting and shredding step, as with ISO 14044. Primary data was directly gathered from the
inventoried in C3. The material leaves the current system at designated person at the relevant production plants. It was
module C3 and enters a subsequent system as a secondary ensured that the collected data accurately represented reality,
fuel. so it can be assumed that the used primary data is of high
quality.
3.3 Estimates and assumptions
Specific, primary data have been used to the highest extent The technological, geographical, and time-related
possible. In case of absence, estimates and assumptions were representativeness of background data (e.g. from EcoInvent)
made to model reality as closely as possible. These was verified, as stated in EN 15804+A2.
assumptions are based on publicly available data and literature.
Generic dataset from the EcoInvent 3.8. database have been 3.7 Period under review
used to model the impact of some raw materials and process- Primary data, needed to calculate the LCA of the system under
related parameters for which specific data was lacking. study, was collected for the year 2020 from the Bazeilles,
BOSPAN, SPANO and Unilin's glue production facility.
End-of-life compact MDF leaves the product system in C3 as a
3.8 Geographic Representativeness
secondary fuel, for which the benefits and loads are inventoried
in module D. Here it is assumed that the secondary fuel Land or region, in which the declared product system is
substitutes electricity and heat in accordance with an average manufactured, used or handled at the end of the product´s
mix available on the European grid. lifespan: Western Europe
3.4 Cut-off criteria
3.9 Allocation
All in- and outputs to the system under study have been
In line with EN 15804+A2 and EN 16485, the biogenic carbon
included in the LCA. Primary data was used to the highest
and primary energy content of the wood have been balanced
extent possible. If primary data was lacking, secondary data
over the product's entire life cycle (A1 - C4) based on its
from EcoInvent was resorted to. Conservative assumptions
inherent material characteristics and underlying physical flows.
were made using average or generic data in case of data gaps.
Fresh wood inventories were taken from EcoIvent 3.8. Here, it
These assumptions are based on publicly available (literature
was made sure that the biogenic carbon and energy content
reported) data. As such, all processes, materials, or emissions
reflect the physical relationships of the different wood-based
expected to have a significant contribution to the environmental
materials.
impact of the system under study were considered in the LCA.
The total sum of omitted flows can therefore be deemed as
The system boundary (and subsequent allocation) relating to
significantly below the 5 % threshold of the system's energy
the flow of the end-of-life product are as described in section
and mass input, as stated in the EN 15804+A2.
3.2.
3.5 Background data
3.10 Comparability
The relevant background data was either taken from the
Basically, a comparison or an evaluation of EPD data is only
EcoInvent 3.8. database or peer-reviewed literature sources.
possible if all the data sets to be compared were created
Measures were taken to ensure that the used secondary data
according to EN 15804 and the building context, respectively
was no more than 10 years old. These data types allowed to
the product-specific characteristics of performance, are taken
map the background system in the LCA of the product under
into account. Background data was used from the EcoInvent
study.
3.8. database.
4. LCA: Scenarios and additional technical information
The end-of-life impact of the used packaging materials is not
Characteristic product properties of biogenic carbon declared. However, its impact can be modelled based on the
The values declared below describe the amount of biogenic data given below.
carbon and stored biogenic CO in the building product under
2 Name Value Unit
study when it leaves the factory gate. These relate to 1 m² of
Wood-based packaging 0.41 kg/m²
Unilin decorative compact MDF (10 mm).
Cardboard 0.004 kg/m²
Biogenic carbon content at factory gate
PET straps 0.0027 kg/m²
The carbon uptake of the packaging materials is not included
Stretch foil 0.00067 kg/m²
below as their end-of-life impact is not declared in module A5.
Information on the reference lifetime can be found in section
Name Value Unit
2.12. Please contact Unilin's sales team or
Biogenic carbon content in product 3.9 kg C/m²
info.panels@unilin.com for more information.
Stored carbon dioxide in product 14.4 kg CO2/m²
End-of-life (C1-C4)
Note: 1 kg biogenic carbon is equivalent to 44/12 kg CO .
2 The following table provides the parameters required to model
the end-of-life of the product under study. Since the product is
not intended for extended outdoor use, it is assumed that its
The following technical information is a basis for the declared moisture content remains consistent with its state at the factory
modules or can be used for developing specific scenarios in the gate. The end-of-life board reaches its end-of-waste state after
context of a building assessment if modules are not declared (preliminary) sorting and shredding. The losses during the
(MND). sorting and shredding are assumed to have a negligible impact
Installation into the building (A5) and are thus discarded. The material leaves the system as a
5 Environmental Product Declaration - Unilin B.V. Division Panels - Unilin Decorative Compact MDF
secondary fuel (energy recovery). The recovery potential is modeled based on the net output flow
Name Value Unit of secondary fuel. It is assumed that a biomass power plant
located in the EU recovers the secondary fuel's energy, with 55
Collected separately 11.15 kg/m²
% of the energy being recovered as heat and the remaining 30
Secondary fuel (output at C3) 11.15 kg/m²
% as electricity. The generated energy carriers are assumed to
substitute heat and electricity in accordance with the average
Reuse, recovery and/or recycling potentials (D)
mix available on the European grid.
In module D, the loads and benefits of exporting the secondary
Name Value Unit
fuel from the system under study are inventoried. The moisture
content of this fuel is assumed to remain consistent with its Net output flow of secondary fuel 10.19 kg/m²
state at factory gate. This value may vary significantly based on Energy efficiency biomass plant 85 %
the storage conditions prior to its intended use.
6 Environmental Product Declaration - Unilin B.V. Division Panels - Unilin Decorative Compact MDF
5. LCA: Results
The values declared below refer to 1 m² of Unilin decorative MDF board with a grammage of 11.15 kg/m² and thickness of 10 mm.
Table "Description of the system boundary" summarizes the scope of the system under study from a life cycle point of view. Declared
modules are indicated with an "X", non-declared modules are indicated with "MND". "MNR" refers to modules which are deemed as not
relevant.
DESCRIPTION OF THE SYSTEM BOUNDARY (X = INCLUDED IN LCA; MND = MODULE OR INDICATOR NOT DECLARED; MNR
= MODULE NOT RELEVANT)
Benefits and
Construction loads beyond
Product stage Use stage End of life stage
process stage the system
boundaries
la ire ta m w a Ry lp p u s tro p s n a rT g n iru tc a fu n a M e h t m o rf tro p s n a rTe tis e h t o t e ta g y lb m e s s A e s U e c n a n e tn ia M ria p e R tn e m e c a lp e R tn e m h s ib ru fe R y g re n e la n o ita re p Oe s u re ta w la n o ita re p Oe s u n o itc u rts n o c -e Dn o itilo m e d tro p s n a rT g n is s e c o rp e ts a W la s o p s iD -e s u e R-y re v o c e R-g n ilc y c e Rla itn e to p
A1 A2 A3 A4 A5 B1 B2 B3 B4 B5 B6 B7 C1 C2 C3 C4 D
X X X MND MND MND MND MNR MNR MNR MND MND X X X X X
RESULTS OF THE LCA - ENVIRONMENTAL IMPACT according to EN 15804+A2: 1 m² Unilin Decorative Compact MDF Board
Parameter Unit A1-A3 C1 C2 C3 C4 D
Global Warming Potential total (GWP-total) kg CO 2 eq -8.71E+00 0 5.02E-02 1.45E+01 0 -7.45E+00
Global Warming Potential fossil fuels (GWP-fossil) kg CO 2 eq 5.62E+00 0 5.01E-02 1.88E-01 0 -7.42E+00
Global Warming Potential biogenic (GWP-biogenic) kg CO 2 eq -1.43E+01 0 1.56E-05 1.44E+01 0 -2.1E-02
Global Warming Potential luluc (GWP-luluc) kg CO 2 eq 1.95E-02 0 1.86E-05 2.56E-04 0 -1.45E-02
Depletion potential of the stratospheric ozone layer (ODP) kg CFC11 eq 1.06E-06 0 1.21E-08 2.7E-08 0 -1.35E-06
Acidification potential of land and water (AP) mol H+ eq 3.57E-02 0 2.11E-04 1.06E-03 0 -1.5E-02
Eutrophication potential aquatic freshwater (EP-freshwater) kg P eq 2.55E-04 0 3.46E-07 1.03E-05 0 -6.42E-04
Eutrophication potential aquatic marine (EP-marine) kg N eq 1.08E-02 0 6.38E-05 2.7E-04 0 5.88E-03
Eutrophication potential terrestrial (EP-terrestrial) mol N eq 1.2E-01 0 7.04E-04 3.02E-03 0 6.2E-02
Formation potential of tropospheric ozone photochemical oxidants kg NMVOC
3.92E-02 0 2.26E-04 8.55E-04 0 1.06E-02
(POCP) eq
Abiotic depletion potential for non fossil resources (ADPE) kg Sb eq 6.72E-05 0 1.2E-07 6.27E-07 0 -2.82E-06
Abiotic depletion potential for fossil resources (ADPF) MJ 1.52E+02 0 7.88E-01 3.41E+00 0 -2.52E+02
m3 world eq
Water use (WDP) 8.17E+00 0 2.67E-03 9.47E-03 0 -1.35E+00
deprived
RESULTS OF THE LCA - INDICATORS TO DESCRIBE RESOURCE USE according to EN 15804+A2: 1 m² Unilin Decorative
Compact MDF Board
Parameter Unit A1-A3 C1 C2 C3 C4 D
Renewable primary energy as energy carrier (PERE) MJ 7.82E+01 0 1E-02 1.5E+02 0 -2.11E+01
Renewable primary energy resources as material utilization
MJ 1.5E+02 0 0 -1.5E+02 0 0
(PERM)
Total use of renewable primary energy resources (PERT) MJ 2.28E+02 0 1E-02 3.62E-01 0 -2.11E+01
Non renewable primary energy as energy carrier (PENRE) MJ 9.57E+01 0 7.88E-01 5.91E+01 0 -2.52E+02
Non renewable primary energy as material utilization (PENRM) MJ 5.62E+01 0 0 -5.57E+01 0 0
Total use of non renewable primary energy resources (PENRT) MJ 1.52E+02 0 7.88E-01 3.41E+00 0 -2.52E+02
Use of secondary material (SM) kg 8.77E-02 0 0 0 0 0
Use of renewable secondary fuels (RSF) MJ 1.17E+01 0 0 0 0 1.16E+02
Use of non renewable secondary fuels (NRSF) MJ 0 0 0 0 0 4.33E+01
Use of net fresh water (FW) m3 2.25E-01 0 9.38E-05 1.9E-03 0 -1.01E-01
RESULTS OF THE LCA – WASTE CATEGORIES AND OUTPUT FLOWS according to EN 15804+A2:
1 m² Unilin Decorative Compact MDF Board
Parameter Unit A1-A3 C1 C2 C3 C4 D
Hazardous waste disposed (HWD) kg 2.13E-01 0 5.46E-04 5.08E-03 0 -1.12E-03
Non hazardous waste disposed (NHWD) kg 2.89E+00 0 7.78E-02 1.4E-01 0 -1.52E+00
Radioactive waste disposed (RWD) kg 5.7E-04 0 5.34E-06 2.38E-05 0 -1E-03
Components for re-use (CRU) kg 0 0 0 0 0 0
Materials for recycling (MFR) kg 0 0 0 0 0 0
Materials for energy recovery (MER) kg 0 0 0 1.12E+01 0 0
Exported electrical energy (EEE) MJ 0 0 0 0 0 0
Exported thermal energy (EET) MJ 0 0 0 0 0 0
RESULTS OF THE LCA – additional impact categories according to EN 15804+A2-optional:
1 m² Unilin Decorative Compact MDF Board
7 Environmental Product Declaration - Unilin B.V. Division Panels - Unilin Decorative Compact MDF
Parameter Unit A1-A3 C1 C2 C3 C4 D
Disease
Incidence of disease due to PM emissions (PM) 3.66E-07 0 5.95E-09 1.25E-08 0 1.11E-07
incidence
Human exposure efficiency relative to U235 (IR) kBq U235 eq 4.5E-01 0 3.42E-03 2.33E-02 0 -1.16E+00
Comparative toxic unit for ecosystems (ETP-fw) CTUe 2.51E-05 0 9.65E-10 4.75E-09 0 -1.63E-08
Comparative toxic unit for humans (carcinogenic) (HTP-c) CTUh 2.69E-08 0 8.08E-12 5.28E-11 0 6.76E-10
Comparative toxic unit for humans (noncarcinogenic) (HTP-nc) CTUh 3.81E-09 0 2.46E-11 1.74E-10 0 -1.13E-09
Soil quality index (SQP) SQP 9.63E+02 0 9.02E-01 1.66E+00 0 -1.96E+01
Disclaimer 1 – for the indicator 'Potential Human exposure efficiency relative to U235'. This impact category deals mainly with the
eventual impact of low-dose ionizing radiation on human health of the nuclear fuel cycle. It does not consider effects due to possible
nuclear accidents, occupational exposure or radioactive waste disposal in underground facilities. Potential ionizing radiation from the
soil, radon and from some construction materials is also not measured by this indicator.
Disclaimer 2 – for the indicators 'abiotic depletion potential for non-fossil resources', 'abiotic depletion potential for fossil resources',
'water (user) deprivation potential, deprivation-weighted water consumption', 'potential comparative toxic unit for ecosystems', 'potential
comparative toxic unit for humans – cancerogenic', 'Potential comparative toxic unit for humans - not cancerogenic', 'potential soil
quality index'. The results of this environmental impact indicator shall be used with care as the uncertainties on these results are high
as there is limited experience with the indicator.
6. LCA: Interpretation
This section aims to analyze and interpret the results of the high wood content (i.e. 70 %) results in a GWP-total of - 8.7
LCA analysis carried for 1 m² of the Unilin decorative compact kg/m². The product thus stores carbon and does not contribute
MDF (10 mm). Although the values for alternative thicknesses to global warming when it leaves Unilin's factory gate. The
can vary from the declared and discussed ones, the observed stored carbon will only be released if the fiberboard can no
trends will be the same throughout the entire product category. longer fulfill its intended purpose (i.e. at end-of-life).
Summary A deep dive in the drivers of the cradle-to-gate environmental
This part intends to summarize the trends observed in the impact shows the significant contribution of the raw materials
cradle-to-gate environmental impact of the Unilin decorative (module A1). 80 % of the fossil CO emissions can primarily be
2
fiberboard. An in-depth analysis is available in the following allocated to the glue and resin production, as well as 97 % of
subsections. the water and 74% of fossil resources used in A1 - A3. The
generation of heat and electricity, required for the decorative
During its growth, wood absorbs CO 2 through photosynthesis MDF production, is an important driver of the production-related
and stores it as biogenic carbon in its biomass. The product's impact. This is observable in the EP-m and POCP indicators.
when the Unilin decorative compact MDF board leaves the
Cradle-to-Cradle Impact - Dominance Analysis factory gate. The product under study thus stores carbon and
The hot-spot analysis highlights the negative GWP-value of does not contribute to global warming.
modules A1 - A3, as depicted in the GWP-focused graph. To
improve the clarity of the graph, the values of the GWP-luluc The stored carbon will only be released when the fiberboard
indicator have been omitted. leaves the system as a secondary fuel. The figure below clearly
demonstrates a neutral biogenic carbon balance in accordance
Wood stores CO as biogenic carbon during its growth (GWP- with EN 16485.
2
biogenic = - 14.3 kg CO eq./m²). This negative GWP-value is
2
The GWP-focused analysis also illustrates the "avoided" impact
partially counterbalanced by the positive GWP-impact of the
(described in module D) related to the export of end-of-life
fossil materials and energy resources used during A1 - A3
fiberboard as a secondary fuel. The energy recovery of that fuel
(GWP-fossil). This results in a GWP-total of - 8.7 kg CO eq./m²
2
8 Environmental Product Declaration - Unilin B.V. Division Panels - Unilin Decorative Compact MDF
generates heat and electricity, which substitutes a European-
averaged mix of heat and electricity from the grid. Since the The hot-spot analysis shows that, for non-GWP-related
largest share of the heat and electricity on the European grid is parameters, modules A1 - A3 are the main contributors to the
fossil-based, a negative GWP-fossil is obtained (i.e. avoided system under study. Values for module D are generally
fossil CO emissions from combustion). It indicates that the negative, except for the EP and POCP indicators. This is
2
combustion of these fossil fuels has a higher impact on global attributed to the emissions from the energy recovery process of
warming than the energy recovery from the secondary fuel. the end-of-life fiberboard.
74 % of all fossil resources used in modules A1 - A3 is allocated
Cradle-to-Grave Impact - Main Drivers to the production of the raw materials (mainly related to the glue
The graph below allows to identify the primary sources of the and resin production).
cradle-to-gate environmental impact. The results show that raw
material production (module A1) has a significant impact. 80 % Energy-related processes are typically the main drivers of the
of the fossil CO emissions are primarily attributed to the environmental impact of module A3. This is observed in the
2
production of the used glue and resin. The contribution of the contribution of A3 to EP-m and POCP, which is traced back to
raw material production is even more significant for the the generation of renewable energy from the woody waste.
indicators ODP, ADPF, ADPE and WDP. 97 % of all water and
9 Environmental Product Declaration - Unilin B.V. Division Panels - Unilin Decorative Compact MDF
7. Requisite evidence
Formaldehyde emissions • Result : 0.01 ppm [Limit < 0.05 ppm]
PCP + Heavy metals + Wood preservative analysis
E1 - EN 13986:2004+A1:2015
• Test report : 1110 As the Unilin melamine faced fibreboard does not contain any
• Method : EN 717-1 post-consumer recycled wood, this evidence is not necessary.
• Product : Melamine faced MDF
• Laboratory : TCNH VOC Emissions
• Result : 0.01 ppm [Limit < 0.1 ppm]
Melamine faced fiberboards are commonly used for interior
E0.5 - ChemVerbotsV building. In many countries national regulations are applicable
for indoor air quality. Please contact Unilin's sales team or
• Test report : 1110
info.panels@unilin.com for more information.
• Method : EN 717-1
• Product : Melamine faced MDF
• Laboratory : TCNH
8. References
Standards
EN 322
ASTM D6007
EN 322:1993, Wood-based panels - Determination of moisture
ASTM D6007:2020, Standard Test Method for Determining content.
Formaldehyde Concentrations in Air from Wood Products Using
a Small-Scale Chamber. EN 323
ASTM E1333 EN 323:2005, Wood-based panels - Determination of density.
ASTM E1333:2020, Standard Test Method for Determining EN 324
Formaldehyde Concentrations in Air and Emission Rates from
Wood Products Using a Large Chamber. EN 324-1:1993, Wood-based panels - Determination of
dimensions of boards - Part 1: Determination of thickness,
EN 310 width and length.
EN 310:1993, Wood-based panels - Determination of modulus EN 622
of elasticity in bending and of bending strength.
EN 622-5:2010, Fibreboards - Specifications - Part 5:
EN 311 Requirements for dry process boards (MDF).
EN 311:2002, Wood-based panels - Surface soundness - Test EN 717-1
method.
EN 717-1:2004, Wood-based panels - Determination of
EN 319 formaldehyde release Formaldehyde emission by the chamber
method
EN 319:1993, Particleboards and fibreboards - Determination
of tensile strength perpendicular to the plane of the board.
10 Environmental Product Declaration - Unilin B.V. Division Panels - Unilin Decorative Compact MDF
EN 12460-5 of dangerous substances - Determination of emissions into
indoor air.
EN 12460-5:2015, Wood-based panels. Determination of
formaldehyde release Extraction method (called the perforator ISO 9001
method).
EN ISO 9001:2008-11, Quality Management Systems –
EN 13501-1 Requirements.
EN 13501-1:2007-05+A1:2009, Fire classification of ISO 14025
construction products and building elements - Part 1:
classification with the results of tests on the reaction to fire of EN ISO 14025:2011, Environmental labels and declarations —
building products. Type III environmental declarations — Principles and
procedures.
EN 13986
ISO 14040
EN 13986:2004+A1:2015, Wood-based panels for use in
construction— Characteristics, valuation of conformity and EN ISO 14040:2006-10, Environmental management — Life
marking cycle assessment — Principles and framework.
EN 14322 ISO 14044
EN 14322:2021, Wood-based panels - Melamine faced boards ISO 14044:2006-10, Environmental management — Life cycle
for interior uses - Definition, requirements and classification. assessment — Principles and framework.
EN 15804 ISO 50001
EN 15804:2012+A2:2019+AC:2021, Sustainability of EN ISO 50001:2018, Energy management systems —
construction works — Environmental Product Declarations — Requirements with guidance for use.
Core rules for the product category of construction products.
JIS A 1460
EN 16000 - 3
JIS A 1460:2021, Building boards Determination of
EN 16000 - 3: 2011, Air sampting on DNPH cartidge and formaldehyde emission -- Desiccator method.
analysis of Iow molecularweight carbonyl compounds by
HPLC/UV JIS A 5908
EN 16000 - 6 JIS A 5908:2022, Particleboards.
EN 16000 - 6: 2012, Air sampling on multiadsorbent (Tenax TA / Additional References
gtass wool) and analysis of volatile organic compounds (VOC)
by TD/cCmS/FID BBSR Table
EN 16000 - 9 BBSR 2017, Useful lives of building components for life cycle
analyses according to the Sustainable Building Assessment
EN 16000 - 9: 2006, lndoor air - Paft 9: Determination of the System, 2017, BBSR Germany 2017.
emission of volatile organic compounds from building products
and furnishing - Emission test chamber method CPR
EN 16000 - 11 CPR EU Ordinance No. 305/2011 of the European Parliament
and Council of 9th March 2011 to define harmonized conditions
EN 16000 - 11: 2006, Indoor air — Part 11: Determination of the for marketing building products.
emission of volatile organic compounds from building products EcoInvent 3.8.
and furnishing — Sampling, storage of samples and
preparation of test specimens. Ecoinvent 3.8, Database for Life Cycle Inventory and
Assessment. Swiss Centre for Life Cycle Inventories, 2021.
EN 16449 Available at: https://ecoinvent.org/the-ecoinvent-database/data-
releases/ecoinvent-3-8/.
EN 16449:2014, Wood and wood-based produts - Calculation
of the biogenic carbon content of wood and conversion to EU Biocidal Products Ordinance No. 528/2012
carbon dioxide.
Regulation (EU) No 528/2012 of the European Parliament and
EN 16485 Council of 22 May 2012 concerning the making available on the
market and use of biocidal products.
EN 16485:2014, Round and sawn timber. Environmental
Product Declarations. Product category rules for wood and EWC
wood-based products for use in consruction.
European Waste Catalogue, Ordinance on the European Waste
EN 16516 Catalogue (Waste Catalogue Ordinance - AVV), reference
Federal Official Journal I 2001, 3379.
EN 16516:2020, Construction products: Assessment of release
11 Environmental Product Declaration - Unilin B.V. Division Panels - Unilin Decorative Compact MDF
IBU 2022
PCR Part B
Institut Bauen und Umwelt e.V.: General Instructions for the
EPD programme of Institut Bauen und Umwelt e.V., Version Product Category Rules for Building-Related Products and
2.1, Berlin: Institut Bauen und Umwelt e.V., 2022 Services. Part B: Requirements on the EPD for Wood based
www.ibu-epd.com panels. Version 2. Berlin: Institut Bauen und Umwelt e.V. (eds.),
2023.
PCR Part A
SVHC List
Product Category Rules for Building-Related Products and
Services. Part A: Calculation Rules for the Life Cycle List of Substances of Very High Concern (SVHC) Candidate for
Assessment and Requirements on the Project Report according Authorisation (ECHA Candidate List), dated 04.07.2023,
to EN 15804+A2:2019. Version 1.3. Berlin: Institut Bauen und published in accordance with Article 59(10) of the REACH
Umwelt e.V. (eds.), 2021. Regulation. Helsinki: European Chemicals Agency.
12 Environmental Product Declaration - Unilin B.V. Division Panels - Unilin Decorative Compact MDF
Publisher
Institut Bauen und Umwelt e.V. +49 (0)30 3087748- 0
Hegelplatz 1 info@ibu-epd.com
10117 Berlin www.ibu-epd.com
Germany
Programme holder
Institut Bauen und Umwelt e.V. +49 (0)30 3087748- 0
Hegelplatz 1 info@ibu-epd.com
10117 Berlin www.ibu-epd.com
Germany
Author of the Life Cycle Assessment
Unilin B.V. Division Panels +32 56 67 52 11
Ooigemstraat 3 info.panels@unilin.com
8710 Wielsbeke https://www.unilinpanels.com/en-
Belgium gb
Owner of the Declaration
Unilin B.V. Division Panels +32 56 66 70 21
Ooigemstraat 3 info.panels@unilin.com
8710 Wielsbeke https://www.unilinpanels.com/en-
Belgium gb
13 Environmental Product Declaration - Unilin B.V. Division Panels - Unilin Decorative Compact MDF
