ENVIRONMENTAL PRODUCT DECLARATION
as per ISO 14025 and EN 15804+A2
Owner of the Declaration VELUX Group
Publisher Institut Bauen und Umwelt e.V. (IBU)
Programme holder Institut Bauen und Umwelt e.V. (IBU)
Declaration number EPD-VEL-20230189-IBA1-EN
Issue date 10.08.2023
Valid to 09.08.2028
VELUX Interior roller blinds - Nature Collection
VELUX A/S
www.ibu-epd.com | https://epd-online.com
1. General Information
VELUX A/S VELUX Interior roller blinds - Nature Collection
Programme holder Owner of the declaration
IBU – Institut Bauen und Umwelt e.V. VELUX Group
Hegelplatz 1 Ådalsvej 99
10117 Berlin 2970 Hørsholm
Germany Denmark
Declaration number Declared product / declared unit
EPD-VEL-20230189-IBA1-EN 1 m² of VELUX interior roller blinds
This declaration is based on the product category rules: Scope:
Sun protection systems, 01.08.2021 100 % of the production volume of the new collection of VELUX interior
(PCR checked and approved by the SVR) roller blinds - Nature Collection produced at the production site in Denmark
(Gåsdal Bygningsindustri A/S), covering the variants DKY and RFY.
The owner of the declaration shall be liable for the underlying information
Issue date and evidence; the IBU shall not be liable with respect to manufacturer
information, life cycle assessment data and evidences.
10.08.2023
The EPD was created according to the specifications of EN 15804+A2. In
the following, the standard will be simplified as EN 15804.
Valid to
09.08.2028 Verification
The standard EN 15804 serves as the core PCR
Independent verification of the declaration and data according to ISO
14025:2011
internally X externally
Dipl.-Ing. Hans Peters
(Chairman of Institut Bauen und Umwelt e.V.)
Florian Pronold Dr. Matthew Fishwick,
(Managing Director Institut Bauen und Umwelt e.V.) (Independent verifier)
1 Environmental Product Declaration - VELUX A/S - VELUX Interior roller blinds - Nature Collection
2. Product
1) 'This product/article/at least one partial article contains
2.1 Product description/Product definition substances listed in the candidate list (date: 02.03.2022)
Manually operated blackout roller blinds (DKY) and translucent exceeding 0.1 percentage by mass:
roller blinds (RFY) are made for installation in VELUX roof
• no
windows. The two VELUX interior roller blinds have been
2) 'This product/article/at least one partial article contains other
developed for optimized environmental performance, e.g.
carcinogenic, mutagenic, reprotoxic (CMR) substances in
related to:
categories 1A or 1B which are not on the candidate list,
• at least 75 % post-consumer recycled aluminum exceeding 0.1 percentage by mass:
• the cloth part of the blinds is made of at least 50%
• not investigated with suppliers
recycled PET
3) 'Biocide products were added to this construction product or
• zero plastic packaging
it has been treated with biocide products (this then concerns a
VELUX interior roller blinds are available in a wide range of
treated product as defined by the (EU) Regulation on Biocidal
colours and designs. In both blinds, the cloth is made of coated
Products No. 528/2012):
polyester. The control bar, top fascia and side rails are made of
anodised or white-painted aluminium. • no
The two blinds are of the size 1178 mm x 780 mm = 0.929 m2
2.6 Manufacture
For the use and application of the product the respective
Extruded aluminium profiles that are either anodised or coated,
national provisions at the place of use apply, in Germany for
are bought from external suppliers. Depending on the size of
example the building codes of the federal states and the
the interior roller blinds, they are either bought cut-to-length or
corresponding national specifications.
as profiles to be cut before assembly. The other parts are also
2.2 Application bought from other internal suppliers or from external suppliers.
The blinds are made for installation in VELUX roof windows. The main production process then consists in assembling the
The VELUX blackout roller blind offers blackout for darkness final product and its packaging before shipment.
anytime. Ideal for bedrooms to ensure a good night's sleep or a
daytime nap. VELUX translucent roller blind provides basic The factories are ISO 9001 certified.
privacy whilst still allowing in natural light. Perfect for living
2.7 Environment and health during manufacturing
rooms, offices and playrooms. The blinds can be combined with
All factories are ISO 14001 and ISO 45001 certified.
exterior sun screening products, electric or solar window
operators and interior insect screens.
2.8 Product processing/Installation
2.3 Technical Data Roller blinds are for installation in VELUX roof windows. It is
easily clicked onto the top brackets pre-fitted on the window,
The declared values in the table relate to the reference product
leaving both hands free during the remaining part of the
DKL (dark variant) in combination with VELUX roof window with
installation.
2-layer insulating glass unit (--70, Uw = 1.3 [W/m2K]). For other
covered product combination specific values please contact 2.9 Packaging
epd.support@velux.com.
The packaging usually consists of:
Name Value Unit - cardboard
U-value reduction ΔU 0.27 W/(m²K) - paper insert
Improved insulation 20 %
The use of other packaging materials is possible, but
Solar energy transmittance (gtot) 0.38 -
insignificant in terms of quantity.
Improved g-value 17 %
Cardboard and paper are usually recycled.
Shading factor (Fc-value) 0.83 -
2.10 Condition of use
Performance data of the product with respect to its
The material composition of VELUX interior roller blinds does
characteristics in accordance with the relevant technical
not change over their service life.
provision (no CE-marking).
2.11 Environment and health during use
2.4 Delivery status
VELUX interior roller blinds do not contain any pollutants that
The product is available in pre-defined sizes covering 0.55 m x
could be released during use.
0.7 m to 1.34 m x 1.6 m.
2.5 Base materials/Ancillary materials Environmental protection: According to current knowledge,
Composition of the VELUX interior roller blind DKY (size 1178 hazards to water, air and soil cannot arise when the products
mm x 780 mm = 0.929 m2): are used as intended.
Aluminium 0.997 kg Health protection: According to current knowledge, no health
Steel 0.060 kg hazards or impairments are to be expected.
Polyester cloth 0.153 kg
2.12 Reference service life
other plastic parts 0.094 kg
It is not possible to calculate the reference service life
according to ISO 15686. The service life based on a
The aluminium profiles contain at least 75 post-consumer
manufacturer's testing is 10 years. The corresponding
recycled aluminium.
utilization scenario is declared in Chapter 4.
The PET part of the cloth is made of at least 50% recycled
bottles.
2.13 Extraordinary effects
2 Environmental Product Declaration - VELUX A/S - VELUX Interior roller blinds - Nature Collection
Fire
Not classified for fire performance. 2.15 Disposal
VELUX interior roller blinds are mostly inert and can be
Water disposed of in an appropriate landfill. However, due to the value
In the event of unforeseen exposure to water (flood), no of the materials or the carbon content of the plastic parts,
adverse effects on human health or the environment are to be recycling or energy recovery is preferable and common.
expected.
Waste code according to the European Waste List (Regulation
Mechanical destruction on the European Waste List):
In the event of unforeseen mechanical destruction, VELUX 17 02 03 plastics
interior roller blinds must be replaced; no adverse effects on 17 04 14 mixed metals
human health or the environment are to be expected.
2.16 Further information
2.14 Re-use phase Further documentation on the products, technical data sheets,
VELUX interior roller blinds can be dismantled manually without BIM files, etc. can be found at:
any problems. The metal parts are usually recycled, and the www.velux.com
plastic parts are sent for thermal recycling for energy recovery.
3. LCA: Calculation rules
products, a mixed end-of-life scenario is modelled, allowing the
3.1 Declared Unit different materials to follow their most likely path. As a rule of
The declared unit for interior roller blinds is 1 m². thumb, metals are recycled and plastics are incinerated (also
Declared unit due to the very limited data availability on plastics recycling and
its benefits). Metals are recycled; it is assumed that these
Name Value Unit
fractions reach the end-of-waste state after having been sorted
Declared unit 1 m2 and transported to a recycler. The combustible material
Grammage 1.4 kg/m2 (plastics) is assumed to be thermally treated in a municipal
waste incineration plant.
In addition to the declared product DKY, the lighter version RFY
(related to the amount of aluminium and cloth) is included in the
Module D includes the benefits and burdens associated with
EPD, hence following a conservative approach for the version
recycling metals beyond the system boundary, resulting from
RFY.
the treatment of recycled materials from the point of end-of-
3.2 System boundary waste to the point of substitution (as loads) and substitution of
primary resources (as benefits).
Type of EPD: Cradle to gate with options, with modules C1 –
It also includes the benefits and burdens associated with
C4, and module D (A1-A3, C1-C3, D and additional modules).
energy recovery from plastic waste in a municipal waste
incineration plant, as modelled in Module C3.
The production of VELUX interior roller blinds (modules A1-
In Module D, only net flows of metals leaving the product
A3) includes raw material extraction, energy generation, waste
system are considered.
treatment and all transports up to the factory gate. In
accordance with COUNCIL REGULATION (EU) No 333/2011,
3.3 Estimates and assumptions
secondary metals are modeled as part of the product system
No further assumptions and estimates relevant to the result had
from the moment they are available as unmixed scrap.
to be made beyond the points made in this chapter 3 and in
Waste or secondary fuels are not used for production.
chapter 4.
Module A4 is not declared due to large variances in transport 3.4 Cut-off criteria
distances between the production site and the construction site,
No data available from the company survey was neglected.
where the product is installed.
These include, among other things, material use, energy
demand (heat, electricity), packaging materials of raw materials
Module A5: The products are delivered to the construction site
(insofar as they are generated as waste) and product
ready to be installed. Manual installation is assumed; electricity
packaging, consumables in production, waste treatment and
consumption related to electric drilling machines, screw drivers,
the transport of all inputs and outputs.
etc. is considered to be negligible. Paper and cardboard are
With this approach, mass and energy flows below 1 % were
recycled; it is assumed that these fractions reach the end-of-
also accounted for. No processes were neglected that would
waste state after having been sorted and transported to a
have been known to the project managers and would have
recycler (as a conservative choice). No packaging waste is
contributed significantly to the indicators of the impact
landfilled.
assessment.
Modules B1 to B7 are not relevant for the product under 3.5 Background data
consideration or no significant environmental impacts occur. Ecoinvent v3.8 (2021, cut-off) was used as the background
database.
Module C1 includes manual dismantling, with no significant
environmental impact. 3.6 Data quality
The foreground data are based on extensive and detailed data
Module C2 comprises the transport of the dismantled VELUX collection at the production site. The foreground data could be
interior roller blind to a sorting plant and then to a waste fully linked with corresponding data records from the
incineration plant for the thermally treated plastic fraction. background database Ecoinvent v3.8 (2021, cut-off).
The background data was updated in 2021. Thus, the quality of
Modules C3/C4: given the complexity of the inventoried the foreground and background data can be rated as very
3 Environmental Product Declaration - VELUX A/S - VELUX Interior roller blinds - Nature Collection
good.
No processes were modelled as part of the foreground model
3.7 Period under review that would have required an allocation of multi-input processes.
The LCA data represents the production conditions for the year Background datasets on municipal waste incineration plants
2021. were taken from ecoinvent without any modification.
3.8 Geographic Representativeness
Allocation of reuse, recycling and recovery was avoided by the
Land or region, in which the declared product system is cut-off approach in the foreground model in line with DIN EN
manufactured, used or handled at the end of the product´s 15804.
lifespan: Europe
3.10 Comparability
Basically, a comparison or an evaluation of EPD data is only
3.9 Allocation
possible if all the data sets to be compared were created
No co-products are generated during the production of the
according to EN 15804 and the building context, respectively
VELUX products. Sorted production scrap of the
the product-specific characteristics of performance, are taken
different metals, notably aluminium, is considered a secondary
into account.
material with no economic value (so no burdens allocated) and
Ecoinvent v3.8 (2021, cut-off) was used as the background
considered in the quantification of net flows leaving the product
database.
system. This approach is chosen to ensure a
coherent quantification of net flows entering module D.
4. LCA: Scenarios and additional technical information
Name Value Unit
Characteristic product properties of biogenic carbon
Reference service life
Information on describing the biogenic carbon content at according to manufacturer's 10 a
factory gate declaration
Name ValueUnit Reference service life - a
kg Declared product properties The product has passed
Biogenic carbon content in product - -
C (at the gate) and finishes internal quality controls.
Biogenic carbon content in accompanying kg Design application
n.a.
packaging C parameters (if instructed by
Installation according to
the manufacturer), including
assembly instructions and -
the references to the
state of the art.
appropriate practices and
Module A5
application codes
The products are delivered to the construction site ready to be
installed. Manual installation is assumed; electricity An assumed quality of Carried out in accordance
consumption related to electric drilling machines, screwdrivers, work, when installed in with the manufacturer's -
etc. is considered to be negligible. accordance with the instructions.
Paper and cardboard are recycled; it is assumed that these manufacturer’s instructions
fractions reach the end-of-waste state after having been sorted Outdoor environment, (for
and transported to a recycler over 150 km with a lorry of 16-32 outdoor applications), e.g.
metric tons, EURO6 (as a conservative choice). weathering, pollutants, UV
Not applicable -
No packaging waste is landfilled. and wind exposure, building
The use of multi-way pallets is not taken into account as orientation, shading,
packaging material. temperature
Indoor environment (for
The declared products are
Reference service life indoor applications), e.g.
intended for installation -
temperature, moisture,
inside a building.
chemical exposure
Usage conditions, e.g. Standard use in any type of
frequency of use, building, i.e. opening/closing -
mechanical exposure 2 times a day
The declared products are
Maintenance e.g. required designed for a reference life
frequency, type and quality of 10 years. They are
-
and replacement of maintained by cleaning water
components at the discretion of the
building occupants.
Module B1
The products are assumed tohave no direct emissions during
the use phase. The indicator values of Module B1 are thus 0.
For biogenic carbon storage, see the table above.
Module B2
For interior roller blinds, no impacts related to maintenance are
inventoried in module B2. Annual cleaning is neglected.
4 Environmental Product Declaration - VELUX A/S - VELUX Interior roller blinds - Nature Collection
Module B6 sorting and 0.437 MJ/kg of diesel fuel for internal logistics are
Interior roller blinds do not consume operational energy. taken into account to disassemble the product. The recovered
material leaves the product system as 'materials for recycling'.
Module C1 The net amounts of the metals leaving the product system are
Manual de-installation is assumed, electricity consumption considered as 'use of secondary material' in Module D.
related to electric screwdrivers, etc. is considered to be
negligible. Thus, no environmental impacts are declared in Module C4
module C1. As stated above, it is assumed that 100 % of the plastic parts
are treated in a waste incineration plant with an efficiency R1
Module C2 < 0.6 (according to the ecoinvent dataset used); 25.57 % of the
Given the complexity of the inventoried products, a mixed end- lower heating value of the plastic parts are recovered as heat
of-life scenario is modelled, allowing the different materials to and 13.0 % as electricity. Recovered energy is reported as
follow their most likely path. It should also be noted that the 'exported energy' and considered in Module D.
deconstruction and waste treatment scenario can vary a lot,
depending on the actual situation. Thus, a generic end-of-life Module D
scenario is assumed. As a rule of thumb, metals are recycled, Module D contains the benefits and loads beyond the system
plastics are incinerated (also due to the very limited availability boundary related to the recycling of metals, which result from
of information on plastics recycling and its benefits). the treatment of recycled materials from the point of end-of-
The combustible material (mainly plastics) is assumed to be waste status to the point of substitution (as loads) and the
transported 50 km with a lorry of 16-32 metric tons, EURO6 to substitution of primary resources (as benefits).
an incineration plant. It also includes the benefits and loads related to the energy
Metals are recycled; it is assumed that these fractions reach the recovery from plastic wastes in a municipal waste incineration
end-of-waste state after having been sorted and transported to plant (MWIP) as modelled in Modules A3, A5 and C3. Due to a
a recycler over 150 km with a lorry of 16-32 metric tons, lack of data for plastics from de-construction activities, the
EURO6. substitution potential of recycled plastics is not taken into
account.
Module C3 Only net flows leaving the product system are considered in
A consumption of 0.03 kWh/kg of electricity for shredding and module D.
5 Environmental Product Declaration - VELUX A/S - VELUX Interior roller blinds - Nature Collection
5. LCA: Results
DESCRIPTION OF THE SYSTEM BOUNDARY (X = INCLUDED IN LCA; ND = MODULE OR INDICATOR NOT DECLARED; MNR =
MODULE NOT RELEVANT)
Benefits and
Construction loads beyond
Product stage Use stage End of life stage
process stage the system
boundaries
la ire ta m w a Ry lp p u s tro p s n a rT g n iru tc a fu n a M e h t m o rf tro p s n a rTe tis e h t o t e ta g y lb m e s s A e s U e c n a n e tn ia M ria p e R tn e m e c a lp e R tn e m h s ib ru fe R y g re n e la n o ita re p Oe s u re ta w la n o ita re p Oe s u n o itc u rts n o c -e Dn o itilo m e d tro p s n a rT g n is s e c o rp e ts a W la s o p s iD -e s u e R-y re v o c e R-g n ilc y c e Rla itn e to p
A1 A2 A3 A4 A5 B1 B2 B3 B4 B5 B6 B7 C1 C2 C3 C4 D
X X X MND X MND MND MNR MNR MNR MND MND X X X X X
RESULTS OF THE LCA - ENVIRONMENTAL IMPACT according to EN 15804+A2: 1 m² VELUX interior roller blind DKY - Nature
Collection
Parameter Unit A1-A3 A5 C1 C2 C3 C4 D
GWP-total kg CO 2 eq 8.18E+00 5.83E-01 0 2.43E-02 4.03E-02 6E-01 -5.3E+00
GWP-fossil kg CO 2 eq 8.74E+00 1.53E-02 0 2.43E-02 2.9E-02 6E-01 -5.29E+00
GWP-biogenic kg CO 2 eq -5.79E-01 5.68E-01 0 0 1.13E-02 0 0
GWP-luluc kg CO 2 eq 1.95E-02 6.21E-06 0 9.88E-06 3.23E-05 1.03E-05 -1.89E-02
ODP kg CFC11 eq 1.2E-06 3.58E-09 0 5.7E-09 1.78E-09 3.56E-09 -1.86E-07
AP mol H+ eq 5.42E-02 8.65E-05 0 1.38E-04 1.11E-04 1.44E-04 -3.3E-02
EP-freshwater kg P eq 3.93E-04 1.12E-07 0 1.79E-07 3.76E-06 3.26E-07 -2.06E-04
EP-marine kg N eq 9.21E-03 3.11E-05 0 4.95E-05 3.55E-05 6.04E-05 -4.93E-03
EP-terrestrial mol N eq 9.5E-02 3.42E-04 0 5.45E-04 4.03E-04 6.56E-04 -5.43E-02
kg NMVOC
POCP 2.76E-02 9.78E-05 0 1.56E-04 1.07E-04 1.67E-04 -1.61E-02
eq
ADPE kg Sb eq 2.14E-04 5.11E-08 0 8.14E-08 5.05E-08 8.63E-08 4.33E-05
ADPF MJ 1.12E+02 2.35E-01 0 3.74E-01 4.01E-01 1.12E-01 -4.9E+01
m3 world eq
WDP 2.88E+00 7.71E-04 0 1.23E-03 9.98E-04 6.75E-03 -6.92E-01
deprived
GWP = Global warming potential; ODP = Depletion potential of the stratospheric ozone layer; AP = Acidification potential of land and water; EP =
Eutrophication potential; POCP = Formation potential of tropospheric ozone photochemical oxidants; ADPE = Abiotic depletion potential for non-fossil
resources; ADPF = Abiotic depletion potential for fossil resources; WDP = Water (user) deprivation potential)
RESULTS OF THE LCA - INDICATORS TO DESCRIBE RESOURCE USE according to EN 15804+A2: 1 m² VELUX interior roller
blind DKY - Nature Collection
Parameter Unit A1-A3 A5 C1 C2 C3 C4 D
PERE MJ 1.61E+01 6.54E+00 0 5.28E-03 5.07E-02 9.47E-03 -6.4E+00
PERM MJ 6.68E+00 -6.53E+00 0 0 -1.46E-01 0 0
PERT MJ 2.28E+01 3.32E-03 0 5.28E-03 -9.5E-02 9.47E-03 -6.4E+00
PENRE MJ 1.04E+02 2.35E-01 0 3.74E-01 3.2E-07 7.52E+00 -4.92E+01
PENRM MJ 7.41E+00 0 0 0 0 -7.41E+00 0
PENRT MJ 1.12E+02 2.35E-01 0 3.74E-01 3.2E-07 1.12E-01 -4.92E+01
SM kg 9.25E-01 0 0 0 0 0 3.42E-01
RSF MJ 0 0 0 0 0 0 0
NRSF MJ 0 0 0 0 0 0 0
FW m3 8.76E-02 2.56E-05 0 4.07E-05 9.57E-05 3E-04 -3.4E-02
PERE = Use of renewable primary energy excluding renewable primary energy resources used as raw materials; PERM = Use of renewable primary
energy resources used as raw materials; PERT = Total use of renewable primary energy resources; PENRE = Use of non-renewable primary energy
excluding non-renewable primary energy resources used as raw materials; PENRM = Use of non-renewable primary energy resources used as raw
materials; PENRT = Total use of non-renewable primary energy resources; SM = Use of secondary material; RSF = Use of renewable secondary fuels;
NRSF = Use of non-renewable secondary fuels; FW = Use of net fresh water
RESULTS OF THE LCA – WASTE CATEGORIES AND OUTPUT FLOWS according to EN 15804+A2:
1 m² VELUX interior roller blind DKY - Nature Collection
Parameter Unit A1-A3 A5 C1 C2 C3 C4 D
HWD kg 9.67E-03 5.99E-07 0 9.53E-07 3.2E-07 4.56E-07 6.64E-04
NHWD kg 2.04E+00 1.57E-02 0 2.51E-02 1.63E-03 1.93E-02 -1.27E+00
RWD kg 6.05E-04 3.39E-06 0 5.4E-06 3.62E-06 7.27E-07 -1.55E-04
CRU kg 0 0 0 0 0 0 0
MFR kg 1.44E-01 3.86E-01 0 0 1.15E+00 0 0
MER kg 0 0 0 0 0 0 0
EEE MJ 2E-02 0 0 0 0 9.63E-01 0
EET MJ 3.93E-02 0 0 0 0 1.89E+00 0
6 Environmental Product Declaration - VELUX A/S - VELUX Interior roller blinds - Nature Collection
HWD = Hazardous waste disposed; NHWD = Non-hazardous waste disposed; RWD = Radioactive waste disposed; CRU = Components for re-use;
MFR = Materials for recycling; MER = Materials for energy recovery; EEE = Exported electrical energy; EET = Exported thermal energy
RESULTS OF THE LCA – additional impact categories according to EN 15804+A2-optional:
1 m² VELUX interior roller blind DKY - Nature Collection
Parameter Unit A1-A3 A5 C1 C2 C3 C4 D
Disease
PM 5.71E-07 1.68E-09 0 2.68E-09 1.75E-09 9.71E-10 -4.28E-07
incidence
IR kBq U235 eq 3.56E-01 1.02E-03 0 1.62E-03 1.39E-03 3.85E-04 -5.84E-02
ETP-fw CTUe 2.54E+02 1.86E-01 0 2.96E-01 2.36E-01 1.48E+00 -1.05E+02
HTP-c CTUh 1.33E-08 7.41E-12 0 1.18E-11 6.37E-12 1.24E-10 -5.94E-09
HTP-nc CTUh 2.74E-07 2.14E-10 0 3.41E-10 2.07E-10 1.06E-09 -8.82E-08
SQP SQP 6.29E+01 2E-01 0 3.19E-01 5.41E-02 3.72E-02 -7.02E+00
PM = Potential incidence of disease due to PM emissions; IR = Potential Human exposure efficiency relative to U235; ETP-fw = Potential comparative
Toxic Unit for ecosystems; HTP-c = Potential comparative Toxic Unit for humans (cancerogenic); HTP-nc = Potential comparative Toxic Unit for humans
(not cancerogenic); SQP = Potential soil quality index
Disclaimer 1 – for the indicator “Potential Human exposure efficiency relative to U235”. This impact category deals mainly with the
eventual impact of low-dose ionizing radiation on human health of the nuclear fuel cycle. It does not consider effects due to possible
nuclear accidents, occupational exposure or radioactive waste disposal in underground facilities. Potential ionizing radiation from the
soil, radon and from some construction materials is also not measured by this indicator.
Disclaimer 2 – for the indicators “abiotic depletion potential for non-fossil resources”, “abiotic depletion potential for fossil resources”,
“water (user) deprivation potential, deprivation-weighted water consumption”, “potential comparative toxic unit for ecosystems”,
“potential comparative toxic unit for humans – cancerogenic”, “Potential comparative toxic unit for humans - not cancerogenic”,
“potential soil quality index”. The results of this environmental impact indicator shall be used with care as the uncertainties on these
results are high as there is limited experience with the indicator.
6. LCA: Interpretation
Figure 1 illustrates the relative contributions of the different are in the order of 20 % to 60% (with the exception of the ODP)
modules along the life cycle of the declared products. of the impacts over the product life cycle (modules A1-C4) and
mainly related to the recycling potential of aluminium.
The use of renewable primary energy is mainly caused by the
share of renewable energy in the electricity mix; thus, the
production stage is the main driver of this impact category; the
same holds also for the use of non-renewable primary energy.
Material use of primary energy is negligible and related to
plastic parts of the product and packaging material. The
material use of primary energy is transferred to its energy use
when the materials containing primary energy are incinerated
with energy recovery.
Non-hazardous waste as the quantitatively most relevant waste
Figure 1: Relative environmental impacts of the different flows is mainly caused in upstream processes (mining and
life cycle stages for the VELUX interior roller blind DKY - processing of aluminium); hazardous and radioactive waste are
Nature Collection (Modules A1-C4 = 100%) mainly caused by the European electricity mix used during the
use phase.
The largest part of environmental impacts is caused during
production (modules A1-A3) of the interior roller blind. The In addition to the declared product DKY, the lighter version RFY
contributions of the other modules of the product life cycle are (related to the amount of aluminium and cloth) is included in the
not significant. EPD. LCAs for these versions have not been calculated
specifically. Hence, no statement can be made on the variance
Benefits and burdens beyond the system boundary (module D) regarding these products.
7. Requisite evidence
7.1 Formaldehyde Not applicable; not tested based on applicable product
Not tested based on applicable product standard. standard.
7.2 MDI 7.4. Fire gas toxicity
Not tested based on applicable product standard. Not tested based on applicable product standard.
7.5 VOC emissions
7.3 Checking of pre-treatment of substances used Not tested based on applicable product standard.
according to AltholzVO
8. References
7 Environmental Product Declaration - VELUX A/S - VELUX Interior roller blinds - Nature Collection
IBU programme documents ISO 45001
ISO 45001:2018-03, Occupational health and safety
IBU (2021) management systems -
IBU (2021): General Instructions for the EPD Programme of the Requirements with guidance for use.
Institut Bauen & Umwelt e.V. (General Instructions for the IBU
EPD Programme). Version 2.0, Institut Bauen & Umwelt, Berlin. ECHA-List
The Candidate List of substances of very high concern,
IBU (2017) available via https://echa.europa.eu/nl/-/four-newsubstances-
IBU (2017): PCR Teil A: PCR Part A: Calculation rules for the added-to-the-candidate-list.
life cycle assessment and requirements for the project report.
Version 1.8., Institut Bauen & Umwelt, Berlin. Regulation on biocidal products
REGULATION (EU) No 528/2012 OF THE EUROPEAN
IBU (2023) PARLIAMENT AND OF THE COUNCIL of 22 May 2012
IBU (2023): PCR Part B: Requirements on the EPD for sun concerning the making available on the market and use of
protection systems. Version 2023/04, Institut Bauen & Umwelt, biocidal products.
Berlin.
Regulation (EU) Nr. 305/2011(CPR)
Standards and legal documents REGULATION (EU) No 305/2011 OF THE EUROPEAN
PARLIAMENT AND OF THE COUNCIL of 9 March 2011 laying
EN 15804 down harmonised conditions for the marketing of construction
EN 15804:2012+A2:2019 + AC:2021, Sustainability of products and repealing Council Directive 89/106/EEC.
construction works - Environmental product declarations - Core
rules for the product category construction products. COUNCIL REGULATION (EU) No 333/2011
COUNCIL REGULATION (EU) No 333/2011 of 31 March 2011
ISO 14025 establishing criteria determining when certain types of scrap
DIN EN ISO 14025:2006-07, Environmental labels and metal cease to be waste under Directive 2008/98/EC of the
declarations - Type III Environmental declarations - Principles European Parliament and of the Council.
and procedures.
European Waste List (Waste index)
ISO 14044 http://www.gesetze-im-internet.de/avv/anlage.htm
DIN EN ISO 14044:2006-07, Environmental management - Life
cycle assessment - Requirements and guidance (ISO Additional references
14044:2006); German and English versions EN ISO
14044:2006. Weidema et al. (2013)
Weidema, B., C. Bauer, R. Hischier, C. Mutel, T. Nemecek, J.
ISO 9001 Reinhard, C.O. Vadenbo, G. Wernet (2013): Overview and
DIN EN ISO 9001:2015, Quality management systems - methodology, Data quality guideline for the ecoinvent database
Requirements. version 3. ecoinvent report no. 1
(v3), St. Gallen, Schweiz.
ISO 14001
DIN EN ISO 14001:2015: Environmental management ecoinvent 3.8
systems - Requirements with guidance for use. ecoinvent 3.8, LCA database, 12/2021. Ecoinvent centre,
Zürich.
8 Environmental Product Declaration - VELUX A/S - VELUX Interior roller blinds - Nature Collection
Publisher
Institut Bauen und Umwelt e.V. +49 (0)30 3087748- 0
Hegelplatz 1 info@ibu-epd.com
10117 Berlin www.ibu-epd.com
Germany
Programme holder
Institut Bauen und Umwelt e.V. +49 (0)30 3087748- 0
Hegelplatz 1 info@ibu-epd.com
10117 Berlin www.ibu-epd.com
Germany
Author of the Life Cycle Assessment
Dr. Frank Werner - Umwelt & Entwicklung + 41 (0)44 241 39 06
Kammelenbergstrasse 30 frank@frankwerner.ch
9011 St. Gallen http://www.frankwerner.ch/
Switzerland
Owner of the Declaration
VELUX Group +4545164726
Ådalsvej 99 jakob.roerbech@velux.com
2970 Hørsholm www.velux.com
Denmark
9 Environmental Product Declaration - VELUX A/S - VELUX Interior roller blinds - Nature Collection
