ENVIRONMENTAL PRODUCT DECLARATION
as per ISO 14025 and EN 15804+A2
Owner of the Declaration VELUX Group
Publisher Institut Bauen und Umwelt e.V. (IBU)
Programme holder Institut Bauen und Umwelt e.V. (IBU)
Declaration number EPD-VEL-20220137-IBJ3-EN
Issue date 25.07.2022
Valid to 24.07.2027
VELUX flat roof window CSP - grid-connected
VELUX A/S
www.ibu-epd.com | https://epd-online.com
1. General Information
VELUX A/S VELUX flat roof window CSP - grid-connected
Programme holder Owner of the declaration
IBU – Institut Bauen und Umwelt e.V. VELUX Group
Hegelplatz 1 Ådalsvej 99
10117 Berlin 2970 Hørsholm
Germany Denmark
Declaration number Declared product / declared unit
EPD-VEL-20220137-IBJ3-EN The declaration represents 1 piece of a grid-connected VELUX flat roof
window CSP of the size 1.20 m
x 1.20 m = 1.44 m2
This declaration is based on the product category rules: Scope:
Windows and doors , 01.08.2021 The declaration covers 100% of grid-connected VELUX flat roof windows
(PCR checked and approved by the SVR) CSP by Partizánske Building Components SK, Slovenia.
The owner of the declaration shall be liable for the underlying information
and evidence; the IBU shall not be liable with respect to manufacturer
Issue date information, life cycle assessment data and evidences.
25.07.2022
The EPD was created according to the specifications of EN 15804+A2. In
the following, the standard will be simplified as EN 15804.
Valid to
Verification
24.07.2027
The standard EN 15804 serves as the core PCR
Independent verification of the declaration and data according to ISO
14025:2011
internally X externally
Dipl.-Ing. Hans Peters
(Chairman of Institut Bauen und Umwelt e.V.)
Florian Pronold Dr. Eva Schmincke,
(Managing Director Institut Bauen und Umwelt e.V.) (Independent verifier)
1 Environmental Product Declaration - VELUX A/S - VELUX flat roof window CSP - grid-connected
2. Product
Name Value Unit
2.1 Product description/Product definition
Reaction to fire - class
The grid-connected Velux flat roof windows CSP consist of a
Resistance to upward load EN 1875 UL 1500 -
motorised (two motors) base unit for smoke ventilation made of
a PVC curb with an integrated glazing unit and a scissor arm water permeability acc. to EN 13985, EN
- class
lifting device for the top unit as well as a one-layer opaque or 1027
transparent acrylic (PMMA) dome. For the placing on the Resistance to downward load EN 1873 UL 2500 -
market of the product in the European Union/European Free Resistance to fire EN 13501-2 NPD -
Trade Association (EU/EFTA) (with the exception of
External fire performance EN 13501-5 NPD -
Switzerland) Regulation (EU) No. 305/2011 (CPR) applies. The
Water tightness EN 1873 passed -
product needs a declaration of performance taking into
consideration EN 1873:2005, Prefabricated accessories for Impact resistance - small hard body passed -
roofing - Individual rooflights of plastics - Product specification passed EN 1873
and test methods, EN 12101-2: Smoke and heat control Impact resistance - large soft body EN
SB 1200 -
systems – Part 2: Specification for natural smoke and heat 1873
exhaust ventilators and the CE-marking. Direct airborne sound insulation EN ISO
33 (-1;-4) dB
For the application and use the respective national provisions 418-3
apply.
Thermal transmittance EN 1873 0,99 W/(m2K)
2.2 Application Luminous transmittance EN 410 0,72 -
Velux flat roof windows CSP are used in renovation and new Air permability EN 1026 4 Class
build. Durability EN 1873 NPD -
Nominal activation system/sensitivity EN
2.3 Technical Data passed -
12101-2
The Declaration of Performance including relevant technical
Response delay (response time) EN
specifications and test methods/test standards can be > 60 s -
12101-2
downloaded from the website www.velux.com/ce.
Re1000 +
Operational reliability EN 12101-2 -
The declared values in the table relate to the reference product 10000
incl. an average pane. For other covered product variants, Aerodynamic free area Aa EN 12101-2 0,64 m2
specific values can be selected at the bottom of the above- Resistance to heat EN 12101-2 B300 Class
mentioned download page
Mechanical stability EN 12101-2 passed -
Donstructional data for CSP 120120 73Q+ISD 0000
Opening under load EN 12101-2 SL 500 Class
For other variants, see velux.com/ce
Low ambient temperature EN 12101-2 T(-15) -
Stability under wind load EN 12101-2 WL 3000 Class
Resistance to wind-induced vibration
NPD -
(where included) EN 12101-2
Performance data of the product in accordance with the
declaration of performance with respect to its essential
characteristics according to
• EN 1873:2005, Prefabricated accessories for roofing -
Individual rooflights of plastics - Product specification
and test methods,
• EN
12101-2, Smoke and heat control systems – Part 2:
Specification for
natural smoke and heat exhaust ventilators.
2.4 Delivery status
The product is available in pre-defined sizes covering 0,6x0,6m
to 1,5x1,5m.
2.5 Base materials/Ancillary materials
Composition of the base unit CSP:
PVC 40 % galvanized steel 10 % stainless steel 7 % wood 8 %
motor 7 % (not inventoried separately) laminated glass 15 %
tempered glass 10 % others
Composition of the top unit (ISD 0000A):
PMMA 95 % iron & cast iron 5 %
1) 'This product/article/at least one partial article contains
substances listed in the candidate list (date: 02.03.2022)
exceeding 0.1 percentage by mass:
• no
2 Environmental Product Declaration - VELUX A/S - VELUX flat roof window CSP - grid-connected
2) 'This product/article/at least one partial article contains other insignificant in terms of quantity.
CMR substances in categories 1A or 1B which are not on the
candidate list, exceeding 0.1 percentage by mass: The plastic packaging (polyethylene (PE) film, polystyrene foam
parts) can be recycled if separated by type; alternatively, they
• not investigated with suppliers
can be incinerated.
3) 'Biocide products were added to this construction product or
it has been treated with biocide products (this then concerns a
2.10 Condition of use
treated product as defined by the (EU) Regulation on Biocidal
The material composition of VELUX flat roof windows does not
Products No. 528/2012):
change over their service life.
• no
2.11 Environment and health during use
Recycled content VELUX flat roof windows do not contain any pollutants that
could be released during use.
Environmental protection: According to current knowledge,
hazards to water, air and soil cannot arise when the products
are used as intended.
The values stated in the table relate to the recycled material Health protection: According to current knowledge, no health
streams in VELUX production. hazards or impairments are to be expected.
2.6 Manufacture 2.12 Reference service life
Base unit: It is not possible to calculate the reference service life
according to ISO 15686. The service life based on a
PVC profiles, gaskets, window opener incl. scissor lifting device manufacturer's declaration is 30 years. The corresponding
and other minor components are produced outside Velux. utilization scenario is declared in 4.
2.13 Extraordinary effects
The insulating glass unit is assembled at the production site in
France. Fire
Minor ABS plastic and glass fibre components are produced at Fire performance according to EN 13501:1
a factory in Denmark.
Name Value
Building material class B
The production and final assembly of the base unit takes place
at the production site in Slovakia. Burning droplets s1
Smoke gas development d0
The final production processes includes preparation of the PVC
frame/sash profiles by cutting, milling and drilling and
Water
installation of EPS foam. The final PVC base is assembled by
In the event of unforeseen exposure to water (flood), VELUX
cutting, deburring and welding, cutting and mounting of gaskets
flat roof windows must be replaced as electrical components;
and installation of glazing unit, window opener incl. gas springs
no adverse effects on human health or the environment are to
be expected.
Top unit:
Mechanical destruction
The plastic dome is produced and assembled at a production
In the event of unforeseen mechanical destruction, VELUX flat
site in Germany.
roof windows must be replaced; apart from potential injuries
from glass cullet, no adverse effects on human health or the
The final production processes include forming/blow moulding
environment are to be expected.
of the plastic dome, with afterwards deburring, engraving and
assembly, as well as packaging, stacking and wrapping of the 2.14 Re-use phase
product on multi-use pallets. The factories are ISO 9001 VVELUX flat roof windows can be dismantled manually without
certified. any problems. The metal parts are usually recycled, and the
plastic parts and wood are sent for thermal recycling for energy
2.7 Environment and health during manufacturing
recovery. Flat glass can be recycled whereas laminated glass is
All factories are ISO 14001 and ISO 45001 certified.
usually used as secondary aggregate in road construction or
landfilling.
2.8 Product processing/Installation
The product is delivered to the customer in two parts, a top and 2.15 Disposal
bottom part. After the hole in the roof is prepared, the bottom
VELUX flat roof windows are mostly inert and can be disposed
part of the product can be installed with the use of a
of in an appropriate landfill. However, due to the value of the
screwdriver, after which the top unit can be fastened to the
materials or the carbon content of the plastic parts and wood,
bottom unit.
recycling or energy recovery is preferable and common.
2.9 Packaging
Waste code according to the European Waste List (Regulation
The packaging usually consists of:
on the European Waste List):
- polyethylene film
- polystyrene foam parts
16 02 14 electronic parts
- cardboard
17 02 01 wood
17 02 02 glass
The use of other packaging materials is possible, but
17 02 03 plastics
3 Environmental Product Declaration - VELUX A/S - VELUX flat roof window CSP - grid-connected
17 04 14 mixed metals Further documentation on the products, technical data sheets,
BIM files, etc. can be found at:
2.16 Further information www.velux.com
3. LCA: Calculation rules
combustible material (plastics, wood, etc.) is assumed to be
3.1 Declared Unit thermally treated in a municipal waste incineration plant.
The declared unit is 1 piece of a grid-connected VELUX flat
roof window CSF with a fixed base unit made of a PVC curb Module D includes the benefits and burdens associated with
with an integrated glazing unit with 1.20 m x 1.20 m = 1.44 m2. recycling metals beyond the system boundary, resulting from
the treatment of recycled materials from the point of end-of-
Declared unit
waste to the point of substitution (as loads) and substitution of
Name Value Unit
primary resources (as benefits).
Declared unit 1 pce. It also includes the benefits and burdens associated with
Area 1.44 m² energy recovery from plastic waste in a municipal waste
Weight 132 kg incineration plant, as modelled in Module C3.
In Module D, only net flows of metals leaving the product
system are considered.
3.2 System boundary
3.3 Estimates and assumptions
Type of EPD: Cradle to gate with options, with modules C1 –
No further assumptions and estimates relevant to the result had
C4, and module D (A1-A3, C1-C3, D and additional modules
to be made beyond the points made in this chapter 3 and in
chapter 4.
The production of VELUX flat roof windows (modules A1-A3)
includes raw material extraction, energy generation, waste 3.4 Cut-off criteria
treatment and all transports up to the factory gate. In No data available from the company survey was neglected.
accordance with COUNCIL REGULATION (EU) No 333/2011, These include, among other things, material use, energy
secondary metals are modeled as part of the product system demand (heat, electricity), packaging materials of raw materials
from the moment they are available as unmixed scrap. (insofar as they are generated as waste) and product
Waste or secondary fuels are not used for production. packaging, consumables in production, waste treatment and
the transport of all inputs and outputs.
Module A4 is not declared due to large variances in transport With this approach, mass and energy flows below 1 % were
distances between the production site and the construction site, also accounted for. No processes were neglected that would
where the product is installed. have been known to the project managers and would have
contributed significantly to the indicators of the impact
Module A5: The products are delivered to the construction site assessment.
ready to be installed. Manual installation is assumed, and
electricity consumption related to electric drilling machines, 3.5 Background data
screw drivers, etc. is considered to be negligible. The Ecoinvent 3.8 (2021) is used as the background database.
combustible packaging material (plastics, wood, etc.) is
assumed to be thermally treated in a municipal waste 3.6 Data quality
incineration plant with an efficiency R1 < 0.6 (according to the The foreground data are based on extensive and detailed data
ecoinvent dataset used); the recovered energy is declared as collection at the production site. The foreground data could be
exported energy. Metals and cardboard are recycled; it is fully linked with corresponding data records from the
assumed that these fractions reach the end-of-waste state after background database ecoinvent 3.8.
having been sorted and transported (as a conservative choice) The background data was updated in 2021. Thus, the quality of
to a recycler. No packaging waste is landfilled. the foreground and background data can be rated as very
good.
Modules B1 to B7 are not relevant for the product under
3.7 Period under review
consideration or no significant environmental impacts occur.
The LCA data represents the production conditions for the year
Module C1 includes manual dismantling, with no significant 2021.
environmental impact.
3.8 Geographic Representativeness
Land or region, in which the declared product system is
Module C2 comprises the transport of the dismantled VELUX
manufactured, used or handled at the end of the product´s
flat roof window to a sorting plant and then to a waste
lifespan: Europe
incineration plant for the thermally treated plastic fraction.
Modules C3/C4: given the complexity of the inventoried
3.9 Allocation
products, a mixed end-of-life scenario is modelled, allowing the
No co-products are generated during the production of the
different materials to follow their most likely path.
VELUX products. Sorted production scrap of the different
As a rule of thumb, metals are recycled and plastics are
metals, notably aluminium, is considered a secondary material
incinerated (also due to the very limited data availability of
with no economic value (so no burdens allocated) and
plastics recycling and its benefits); coated and uncoated flat
considered in the quantification of net flows leaving the product
glass is assumed to be recycled whereas laminated glass is
system. This approach is chosen to ensure a coherent
assumed to be landfilled due to very limited recycling potential.
quantification of net flows entering module D.
Metals and flat glass recycled; it is assumed that these fractions
Biogenic carbon is allocated based on physical flows
reach an end-of-waste state after having been sorted and
regardless of the allocation procedure chosen for the process.
transported to a recycler; laminated glass is landfilled. The
The biogenic carbon content of wood products entering or
4 Environmental Product Declaration - VELUX A/S - VELUX flat roof window CSP - grid-connected
leaving the product system is quantified (manually) as part of cut-off approach in the foreground model in line with DIN EN
the GWP in conformity with DIN EN 16485. 15804.
No processes were modelled as part of the foreground model 3.10 Comparability
that would have required an allocation of multi-input processes. Basically, a comparison or an evaluation of EPD data is only
Background datasets on municipal waste incineration plants possible if all the data sets to be compared were created
were taken from ecoinvent without any modification. according to EN 15804 and the building context, respectively
the product-specific characteristics of performance, are taken
Allocation of reuse, recycling and recovery was avoided by the into account.
4. LCA: Scenarios and additional technical information
Name Value Unit
Characteristic product properties of biogenic carbon
Reference service life
according to
30 a
Information on describing the biogenic carbon content at manufacturer's
factury gate declaration
Name ValueUnit The product has passed
Declared product
kg internal quality controls and
Biogenic carbon content in product 4.38 properties (at the gate) -
C complies with EN 1873 for CE
and finishes
marking
Biogenic carbon content in accompanying kg
2.77
packaging C Design application
parameters (if instructed
Note: 1 kg of biogenic carbon is equivalent to 44/12 kg of CO .
2 by the manufacturer), Installation according to
including the references assembly instructions and -
to the appropriate state of the art.
practices and application
codes
An assumed quality of
Module A5
work, when installed in
The products are delivered to the construction site ready to be Carried out in accordance with
accordance with the -
installed. Manual installation is assumed, and electricity the manufacturer's instructions.
manufacturer’s
consumption related to electric drilling machines, screw drivers,
instructions
etc. is considered to be negligible.
Outdoor environment, (for The declared products are
The combustible packaging material (plastics, wood, etc.) is
outdoor applications), e.g. intended for installation outside
assumed to be transported 50 km with a lorry 16-32 metric
weathering, pollutants, UVthe building: They are therefore
tons, EURO6 to an incineration plant with an efficiency R1 < 0.6 -
and wind exposure, designed to withstand outdoor
(according to the ecoinvent dataset used); the recovered
building orientation, conditions throughout their
energy is declared as exported energy; for its quantification an
shading, temperature service life.
efficiency of 25.6 % is assumed for the production of heat and
13.0 % for the production of electricity (always referring to the Indoor environment (for
The declared products are not
lower heating value of the waste). indoor applications), e.g.
intended for installation inside -
Metals and cardboard are recycled; it is assumed that these temperature, moisture,
a building.
fractions reach the end-of-waste state after having been sorted chemical exposure
and transported (as a conservative choice) to a recycler over Usage conditions, e.g. Standard use in any type of
150 km with a lorry 16-32 metric tons, EURO6. frequency of use, building, i.e. opening/closing -
No packaging waste is landfilled. mechanical exposure as often as necessary.
The use of multi-way pallets is not taken into account as The declared products are
packaging material. designed for a reference life of
Maintenance e.g. required
30 years, with the motor
frequency, type and
Reference service life replaced every 15 years. They -
quality and replacement
are maintained by cleaning
of components
water at the discretion of the
building occupants.
Module B1
The products are assumed to have no direct emissions during
the use phase. The indicator values of Module B1 are thus 0.
For biogenic carbon stored in product, see above.
Module B2
The maintenance scenario (B2) covers the replacement of the
motor over the service life of the product. Given that the
detailed composition of the motor and its electronic
components is not known, potential loads and benefits related
to the motor and electronics are disregarded.
Annual cleaning with water (e.g., using 1 l/m2 of tap water per
annual cleaning) is neglected.
5 Environmental Product Declaration - VELUX A/S - VELUX flat roof window CSP - grid-connected
Module B6
For motor-operated flat roof windows, electricity is used both in Module C4
stand-by and during operations. As stated above, it is assumed that 100 % of the plastic parts
and the wooden parts are treated in a waste incineration plant
Module C1 with an efficiency R1 < 0.6 (according to the ecoinvent dataset
Manual de-installation is assumed, electricity consumption used); 25.57 % of the lower heating value of the plastic parts
related to electric screw drivers, etc. is considered to be are recovered as heat and 13.0 % as electricity. Recovered
negligible. Thus, no environmental impacts are declared in energy is reported as 'exported energy' and considered in
module C1. Module D.
Module C2 Some of the material, notably laminated flat glass is assumed
Given the complexity of the inventoried products, a mixed end- to be landfilled.
of-life scenario is modelled, allowing the different materials to
follow their most likely path. Module D
Module D contains the benefits and loads beyond the system
It should also be noted that the deconstruction and waste boundary related to the recycling of metals, which result from
treatment scenario can vary a lot, depending on the actual the treatment of recycled materials from the point of end-of-
situation. Thus, a generic end-of-life scenario is assumed. waste status to the point of substitution (as loads) and the
substitution of primary resources (as benefits).
As a rule of thumb, metals are recycled, plastics are incinerated
(also due to the very limited availability on plastics recycling Furthermore, it includes the benefits of raw material substitution
and its benefits); coated and uncoated flat glass is assumed to of the recycling of flat glass, with the exception of laminated
be recycled whereas laminated glass is assumed to be glass, which cannot be used for the production of glass again.
landfilled due to very limited recycling potential. Recovered flat glass is assumed to have reached the end-of-
waste state as sorted glass cullet; glass cullet is assumed to
The combustible material (plastics, wood, etc.) is assumed to replace virgin raw material for glass production – impacts on
be transported 50 km with a lorry 16-32 metric tons, EURO6 to the energy required to remelt recycled glass as compared to
an incineration plant. virgin glass production are neglected due to a lack of data.
Metals and flat glass recycled; it is assumed that these fractions It also includes the benefits and loads related to the energy
reach the end-of-waste state after having been sorted and recovery from plastic wastes in a MWIP as modelled in
transported to a recycler over 150 km with a lorry 16-32 metric Modules A3, A5 and C3.
tons, EURO6.
The benefits of the recycling of the motor and electronic parts
Laminated glass is landfilled, including a transport of 30 km with are not considered due to the absence of data on its
a lorry 16-32 metric tons, EURO6. composition and recycled content.
Module C3 Due to a lack of data for plastics from de-construction activities,
A consumption of 0.03 kWh/kg of electricity for shredding and the substitution potential of recycled plastics is not taken into
sorting and 0.437 MJ/kg of diesel fuel for internal logistics are account.
taken into account to disassemble the product. The recovered
material leaves the product system as 'materials for recycling'. Only net flows leaving the product system are considered in
The net amounts of the metals leaving the product system are module D.
considered as 'use of secondary material' in Module D.
6 Environmental Product Declaration - VELUX A/S - VELUX flat roof window CSP - grid-connected
5. LCA: Results
Disclaimer:
EP-freshwater: This indicator has been calculated as 'kg P eq' as required in the characterization model (EUTREND model, Struijs et
al., 2009b, as implemented in ReCiPe; http://eplca.jrc.ec.europa.eu/LCDN/developerEF.xhtml)
DESCRIPTION OF THE SYSTEM BOUNDARY (X = INCLUDED IN LCA; MND = MODULE OR INDICATOR NOT DECLARED; MNR
= MODULE NOT RELEVANT)
Benefits and
Construction loads beyond
Product stage Use stage End of life stage
process stage the system
boundaries
la ire ta m w a Ry lp p u s tro p s n a rT g n iru tc a fu n a M e h t m o rf tro p s n a rTe tis e h t o t e ta g y lb m e s s A e s U e c n a n e tn ia M ria p e R tn e m e c a lp e R tn e m h s ib ru fe R y g re n e la n o ita re p Oe s u re ta w la n o ita re p Oe s u n o itc u rts n o c -e Dn o itilo m e d tro p s n a rT g n is s e c o rp e ts a W la s o p s iD -e s u e R-y re v o c e R-g n ilc y c e Rla itn e to p
A1 A2 A3 A4 A5 B1 B2 B3 B4 B5 B6 B7 C1 C2 C3 C4 D
X X X MND X X X MNR MNR MNR X MND X X X X X
RESULTS OF THE LCA - ENVIRONMENTAL IMPACT according to EN 15804+A2: 1 piece VELUX flat roof window CSP - grid-
connected, 1.20 m x 1.20 m = 1.44 m2
Parameter Unit A1-A3 A5 B1 B2 B6 C1 C2 C3 C4 D
GWP-total kg CO 2 eq 3.89E+02 1.21E+01 0 5.2E+01 6.87E+02 0 1.21E+00 1.23E+01 1.55E+02 -8.24E+01
GWP-fossil kg CO 2 eq 4.15E+02 1.97E+00 0 5.19E+01 6.85E+02 0 1.21E+00 1.22E+01 1.39E+02 -8.24E+01
GWP-
biogenic kg CO 2 eq -2.62E+01 1.02E+01 0 0 0 0 0 8.53E-02 1.6E+01 0
GWP-luluc kg CO 2 eq 4.38E-01 1.17E-04 0 7.52E-02 1.71E+00 0 4.92E-04 3.43E-03 5.33E-02 -6.41E-02
ODP kg CFC11 eq 8.87E-05 6.69E-08 0 2.39E-06 3.47E-05 0 2.84E-07 2.13E-07 1.82E-05 -5.74E-06
AP mol H+ eq 2.52E+00 1.78E-03 0 7.98E-01 3.53E+00 0 6.86E-03 1.4E-02 1.99E-01 -2.32E-01
EP-
kg P eq 1.62E-02 2.21E-06 0 3.96E-03 7.69E-02 0 8.9E-06 3.66E-04 1.58E-03 -5.91E-03
freshwater
EP-marine kg N eq 3.95E-01 6.57E-04 0 6.29E-02 4.52E-01 0 2.47E-03 4.83E-03 4.38E-02 -4.14E-02
EP-terrestrial mol N eq 4.35E+00 7.27E-03 0 7.85E-01 5.23E+00 0 2.71E-02 5.31E-02 4.83E-01 -4.84E-01
kg NMVOC
POCP 1.41E+00 2.06E-03 0 2.5E-01 1.43E+00 0 7.76E-03 1.39E-02 1.3E-01 -1.51E-01
eq
ADPE kg Sb eq 5.38E+02 9.72E-07 0 1.49E-02 1.66E-03 0 4.05E-06 5.83E-06 4.21E-04 -8.73E-04
ADPF MJ 5.93E+03 4.38E+00 0 4.74E+02 1.45E+04 0 1.86E+01 4.24E+01 4.03E+02 -1.13E+03
m3 world eq
WDP 1.79E+02 1.68E-02 0 2.02E+01 1.62E+02 0 6.11E-02 6.54E-01 3E+01 -8.16E+00
deprived
GWP = Global warming potential; ODP = Depletion potential of the stratospheric ozone layer; AP = Acidification potential of land and water; EP =
Eutrophication potential; POCP = Formation potential of tropospheric ozone photochemical oxidants; ADPE = Abiotic depletion potential for non-fossil
resources; ADPF = Abiotic depletion potential for fossil resources; WDP = Water (user) deprivation potential)
RESULTS OF THE LCA - INDICATORS TO DESCRIBE RESOURCE USE according to EN 15804+A2: 1 piece VELUX flat roof
window CSP - grid-connected, 1.20 m x 1.20 m = 1.44 m2
Parameter Unit A1-A3 A5 B1 B2 B6 C1 C2 C3 C4 D
PERE MJ 7.52E+02 6.52E-02 0 5.89E+01 2.75E+03 0 2.63E-01 5.09E+00 2.12E+02 -1.26E+02
PERM MJ 2.85E+02 -1.17E+02 0 0 0 0 0 -1.1E+00 -1.67E+02 0
PERT MJ 1.04E+03 -1.17E+02 0 5.89E+01 2.75E+03 0 2.63E-01 3.99E+00 4.55E+01 -1.26E+02
PENRE MJ 5.34E+03 3.02E+01 0 4.75E+02 1.46E+04 0 1.86E+01 4.26E-05 1.65E+03 -1.14E+03
PENRM MJ 1.27E+03 -2.58E+01 0 0 0 0 0 0 -1.24E+03 0
PENRT MJ 6.61E+03 4.38E+00 0 4.75E+02 1.46E+04 0 1.86E+01 4.26E-05 4.05E+02 -1.14E+03
SM kg 2.92E+01 0 0 0 0 0 0 0 0 8.43E+00
RSF MJ 0 0 0 0 0 0 0 0 0 0
NRSF MJ 0 0 0 0 0 0 0 0 0 0
FW m3 4.02E+00 7.63E-04 0 4.78E-01 9.35E+00 0 2.03E-03 1.72E-02 7.86E-01 -2.5E-01
PERE = Use of renewable primary energy excluding renewable primary energy resources used as raw materials; PERM = Use of renewable primary
energy resources used as raw materials; PERT = Total use of renewable primary energy resources; PENRE = Use of non-renewable primary energy
excluding non-renewable primary energy resources used as raw materials; PENRM = Use of non-renewable primary energy resources used as raw
materials; PENRT = Total use of non-renewable primary energy resources; SM = Use of secondary material; RSF = Use of renewable secondary fuels;
NRSF = Use of non-renewable secondary fuels; FW = Use of net fresh water
RESULTS OF THE LCA – WASTE CATEGORIES AND OUTPUT FLOWS according to EN 15804+A2:
1 piece VELUX flat roof window CSP - grid-connected, 1.20 m x 1.20 m = 1.44 m2
Parameter Unit A1-A3 A5 B1 B2 B6 C1 C2 C3 C4 D
HWD kg 4.47E-02 1.14E-05 0 1.97E-02 5.15E-03 0 4.75E-05 4.26E-05 6.8E-04 -1.62E-03
NHWD kg 1.68E+02 3.08E-01 0 2.41E+01 5.46E+01 0 1.25E+00 4.74E+00 4.17E+01 -3.55E+01
7 Environmental Product Declaration - VELUX A/S - VELUX flat roof window CSP - grid-connected
RWD kg 3E-02 6.26E-05 0 2.37E-03 1.95E-01 0 2.69E-04 3.77E-04 3.04E-03 -4.56E-03
CRU kg 0 0 0 0 0 0 0 0 0 0
MFR kg 1.63E+01 6.91E+00 0 0 0 0 0 3.21E+01 0 0
MER kg 0 0 0 0 0 0 0 0 0 0
EEE MJ 1.44E+01 3.35E+00 0 0 0 0 0 0 1.84E+02 0
EET MJ 2.82E+01 6.6E+00 0 0 0 0 0 0 3.61E+02 0
HWD = Hazardous waste disposed; NHWD = Non-hazardous waste disposed; RWD = Radioactive waste disposed; CRU = Components for re-use;
MFR = Materials for recycling; MER = Materials for energy recovery; EEE = Exported electrical energy; EET = Exported thermal energy
RESULTS OF THE LCA – additional impact categories according to EN 15804+A2-optional:
1 piece VELUX flat roof window CSP - grid-connected, 1.20 m x 1.20 m = 1.44 m2
Parameter Unit A1-A3 A5 B1 B2 B6 C1 C2 C3 C4 D
Disease
PM 2.08E-05 2.66E-08 0 3.9E-06 9.01E-06 0 1.09E-07 1.83E-07 1.53E-06 -2.18E-06
incidence
IR kBq U235 eq 1.17E+01 1.89E-02 0 1.24E+00 1.32E+02 0 8.09E-02 1.48E-01 1.75E+00 -2.03E+00
ETP-fw CTUe 1.43E+04 4.27E+00 0 5.84E+03 7.3E+03 0 1.47E+01 7.99E+01 7.6E+03 -1.15E+03
HTP-c CTUh 2.07E-06 3.44E-10 0 2.52E-07 1.95E-07 0 5.88E-10 1.41E-09 4.93E-08 -4.23E-07
HTP-nc CTUh 1.6E-05 5.52E-09 0 9.13E-06 6.34E-06 0 1.7E-08 1.45E-07 1.9E-06 -2.32E-07
SQP SQP 4.76E+03 3.7E+00 0 3.18E+02 2.23E+03 0 1.59E+01 7.67E+00 1.25E+02 -1.99E+02
PM = Potential incidence of disease due to PM emissions; IR = Potential Human exposure efficiency relative to U235; ETP-fw = Potential comparative
Toxic Unit for ecosystems; HTP-c = Potential comparative Toxic Unit for humans (cancerogenic); HTP-nc = Potential comparative Toxic Unit for humans
(not cancerogenic); SQP = Potential soil quality index
Disclaimer 1 – for the indicator 'Potential Human exposure efficiency relative to U235'.This impact category deals mainly with the
eventual impact of low dose ionizing radiation on human health of the nuclear fuel cycle. It does not consider effects due to possible
nuclear accidents, occupational exposure or radioactive waste disposal in underground facilities. Potential ionizing radiation from the
soil, radon and from some construction materials is also not measured by this indicator.
Disclaimer 2 – for the indicators 'abiotic depletion potential for non-fossil resources', 'abiotic depletion potential for fossil resources',
'water (user) deprivation potential, deprivation-weighted water consumption', 'potential comparative toxic unit for ecosystems', 'potential
comparative toxic unit for humans – cancerogenic', 'Potential comparative toxic unit for humans - not cancerogenic', 'potential soil
quality index'. The results of this environmental impact indicator shall be used with care as the uncertainties on these results are high
as there is limited experience with the indicator.
6. LCA: Interpretation
Figure 1 illustrates the relative contributions of the different
modules along the life cycle of the declared products.
Benefits and burdens beyond the system boundary (module D)
Figure 1: Relative environmental impacts of the different are comparably small (around 10% of the impacts over the
life cycle stages for the flat roof window CSP mains product life cycle (modules A1-C4)). [1]
The largest part of environmental impacts – between 17 % and The use of renewable primary energy is mainly caused by the
rather 100 % - is caused during production (modules A1-A3) of share of renewable energy in the electricity mix, thus the
the flat roof window. Operational energy – i.e., the generation production stage and the use of operational energy are the
electricity used during the use phase - is the most dominant main drivers of this impact category; for the use of non-
contributor in several impact categories. renewable primary energy, the operational energy use is the
8 Environmental Product Declaration - VELUX A/S - VELUX flat roof window CSP - grid-connected
most impacting life cycle stage (around double the impact from Non-hazardous waste as the quantitatively most relevant waste
production). flows is mainly caused during the production of the glass and
during disposal of the product; hazardous and radio-active
Material use of primary energy is negligible and related to wastes are mainly caused by the European electricity mix.
plastic parts of the product and packaging material. The
material use of primary energy is transferred to its energy use [1] Benefits resulting from the recycling of plastics as well as
when the materials containing primary energy are incinerated from the recycling of the electronic parts are disregarded due to
with energy recovery. the lack of data on the recycling processes and related to the
detailed composition of the electronic parts.
7. Requisite evidence
to AltholzVO
8.1 Formaldehyde Not applicable; not tested based on applicable product
Not tested based on applicable product standard. standard. 7.4. Fire gas toxicity
Not tested based on applicable product standard. 7.5 VOC
7.2 MDI emissions
Not tested based on applicable product standard. 7.3 Not tested based on applicable product standard.
Checking of pre-treatment of substances used according
8. References
Product category rules of IBU Individual rooflights of plastics - Product specification and test
methods.
IBU (2021)
IBU (2021): General Instructions for the EPD Programme of the EN 12101-2
Institut Bauen & Umwelt e.V. (General Instructions for the IBU DIN EN 12101-2:2017-08, Smoke and heat control systems –
EPD Programme). Version 2.0, Institut Bauen & Umwelt, Berlin Part 2: Specification for natural smoke and heat exhaust
ventilators.
IBU (2017)
IBU (2017): PCR Teil A: PCR Part A: Calculation rules for the EN 16485
life cycle assessment and requirements for the project report. DIN EN 16485:2014-07, Round and sawn timber -
Version 1.8., Institut Bauen & Umwelt, Berlin. Environmental Product Declarations - Product category rules
for wood and wood-based products for use in construction;
IBU (2021) German version EN 16485:2014.
IBU (2021):PCR Part B: Requirements on the EPD for windows
and doors. Version 2021/01, Institut Bauen & Umwelt, Berlin. ECHA-List
The Candidate List of substances of very high concern,
Standards and legal documents available via https://echa.europa.eu/nl/-/four-newsubstances-
added-to-the-candidate-list.
EN 15804
DIN EN 15804+A2:2019, Sustainability of construction works - Regulation on biocidal products
Environmental product declarations - Core rules for the product REGULATION (EU) No 528/2012 OF THE EUROPEAN
category construction products. PARLIAMENT AND OF THE COUNCIL of 22 May 2012
concerning the making available on the market and use of
ISO 14025 biocidal products.
DIN EN ISO 14025:2006-07, Environmental labels and
declarations - Type III Environmental declarations - Principles Regulation (EU) Nr. 305/2011(CPR)
and procedures. REGULATION (EU) No 305/2011 OF THE EUROPEAN
PARLIAMENT AND OF THE COUNCIL of 9 March 2011 laying
ISO 14044 down harmonised conditions for the marketing of construction
DIN EN ISO 14044:2006-07, Environmental management - Life products and repealing Council Directive 89/106/EEC.
cycle assessment - Requirements and guidance (ISO
14044:2006); German and English versions EN ISO COUNCIL REGULATION (EU) No 333/2011
14044:2006. COUNCIL REGULATION (EU) No 333/2011 of 31 March 2011
establishing criteria determining when certain types of scrap
ISO 9001 metal cease to be waste under Directive 2008/98/EC of the
DIN EN ISO 9001:2015, Quality management systems - European Parliament and of the Council.
Requirements.
European Waste List (Waste index)
ISO 14001 http://www.gesetze-im-internet.de/avv/anlage.htm
DIN EN ISO 14001:2015: Environmental management
systems - Requirements with guidance for use. Additional references
ISO 45001 Weidema et al. (2013)
ISO 45001:2018-03, Occupational health and safety Weidema, B., C. Bauer, R. Hischier, C. Mutel, T. Nemecek, J.
management systems - Requirements with guidance for use. Reinhard, C.O. Vadenbo, G. Wernet (2013): Overview and
methodology, Data quality guideline for the ecoinvent database
EN 1873 version 3. ecoinvent report no. 1 (v3), St. Gallen, Schweiz.
DIN EN 1873:2005, Prefabricated accessories for roofing -
9 Environmental Product Declaration - VELUX A/S - VELUX flat roof window CSP - grid-connected
ecoinvent 3.8 Zürich.
ecoinvent 3.8, LCA database, 12/2021. Ecoinvent centre,
10 Environmental Product Declaration - VELUX A/S - VELUX flat roof window CSP - grid-connected
Publisher
Institut Bauen und Umwelt e.V. +49 (0)30 3087748- 0
Hegelplatz 1 info@ibu-epd.com
10117 Berlin www.ibu-epd.com
Germany
Programme holder
Institut Bauen und Umwelt e.V. +49 (0)30 3087748- 0
Hegelplatz 1 info@ibu-epd.com
10117 Berlin www.ibu-epd.com
Germany
Author of the Life Cycle Assessment
Dr. Frank Werner - Umwelt & Entwicklung + 41 (0)44 241 39 06
Kammelenbergstrasse 30 frank@frankwerner.ch
9011 St. Gallen http://www.frankwerner.ch/
Switzerland
Owner of the Declaration
VELUX Group +4545164726
Ådalsvej 99 jakob.roerbech@velux.com
2970 Hørsholm www.velux.com
Denmark
11 Environmental Product Declaration - VELUX A/S - VELUX flat roof window CSP - grid-connected
