ENVIRONMENTAL PRODUCT DECLARATION
as per ISO 14025 and EN 15804+A2
Owner of the Declaration VELUX Group
Publisher Institut Bauen und Umwelt e.V. (IBU)
Programme holder Institut Bauen und Umwelt e.V. (IBU)
Declaration number EPD-VEL-20230510-CBJ2-EN
Issue date 11.03.2024
Valid to 10.03.2029
VELUX wooden roof windows (triple glazing configuration)
VELUX Group
www.ibu-epd.com | https://epd-online.com
General Information
VELUX Group VELUX wooden roof windows (triple glazing
configuration)
Programme holder Owner of the declaration
IBU – Institut Bauen und Umwelt e.V. VELUX Group
Hegelplatz 1 Ådalsvej 99
10117 Berlin 2970 Hørsholm
Germany Denmark
Declaration number Declared product / declared unit
EPD-VEL-20230510-CBJ2-EN The declared unit is a wooden roof window of 1 m2 with triple glazing
configuration (3-layer). The declared unit is based on the size 1.34 m x
1.40 m (UK08), which is the closest available size to the standard size 1.23
m x 1.48 m (DS/EN 17213:2020).
This declaration is based on the product category rules: Scope:
Windows and doors , 01.08.2021 The EPD is a representative EPD covering VELUX wooden roof windows
(PCR checked and approved by the SVR) as specified in more detail in the product description. The products are
manufactured by the VELUX Group at production sites in different
locations in Europe for sale throughout Europe. The windows' production
Issue date take place in Poland, Denmark, France and Germany.
The owner of the declaration shall be liable for the underlying information
11.03.2024
and evidence; the IBU shall not be liable with respect to manufacturer
information, life cycle assessment data and evidences.
Valid to
The EPD was created according to the specifications of EN 15804+A2. In
10.03.2029 the following, the standard will be simplified as EN 15804.
Verification
The standard EN 15804 serves as the core PCR
Independent verification of the declaration and data according to ISO
14025:2011
internally X externally
Dipl.-Ing. Hans Peters
(Chairman of Institut Bauen und Umwelt e.V.)
Florian Pronold Dr.-Ing. Nikolay Minkov,
(Managing Director Institut Bauen und Umwelt e.V.) (Independent verifier)
1 Environmental Product Declaration - VELUX Group - VELUX wooden roof windows (triple glazing configuration)
Product
Product description/Product definition
The VELUX wooden roof windows are skylight window products
for sale in the European market. The product family covers a
range of product varieties as specified in the table below. All
windows have a wooden frame/sash. Some windows can be
opened (venting), while others cannot be opened (fixed). In
addition, the windows consist of 4 different hinge-functionalities
(pivot-hung, top-hung, side-hung, bottom-hung). The handles
and handlebars are made of aluminium, while the hinges are
made of steel (galvanised, stainless). Some of the window
varieties can be used in conjunction with electric or solar
window operators for automatic opening and closing, while
other windows are opened and closed manually. The
calculations are based on the representative window type
named GPL. In the LCA, the GPL was assessed to be a
conservative choice for a representative window type.
The glass panes are with triple glazing (3-layer glazing unit)
and different glass configurations are covered by the EPD. The
glass thickness ranges from 10 to 13 mm. The glass panes
have cavities filled with Krypton gas. The EPD is based on an
average of the included glazing unit configurations. The
included glazing unit configurations are: 15, 61, 64, 66 (86), 67,
68 and 69.
Only the window modules are included, which means that any
applied window operators, installation products, accessories,
etc. are not part of the EPD. These are available as separate
EPDs, that can be used in combination with this EPD.
1 3-layer glazing options: 15, 61, 64, 66 (86), 67, 68, 69
For the placing on the market of the product in the European
Union/European Free Trade Association (EU/EFTA) (with the
exception of Switzerland) Regulation (EU) No. 305/2011 (CPR)
applies. The product needs a declaration of performance taking
into consideration EN 14351-1:2006+A2:2016, Windows and
doors - Product standard, performance characteristics - Part 1:
Windows and external pedestrian doorsets. For the application
and use, the respective national provisions apply.
Application
VELUX wooden roof windows are used in renovation and new
build. Either installed as a single window or in a combination of
multiple windows.
Technical Data
The Declaration of Performance including relevant technical
specifications and test methods/test standards can be
downloaded from the website www.velux.com/ce
2 Environmental Product Declaration - VELUX Group - VELUX wooden roof windows (triple glazing configuration)
The performance values are specific for each standard wooden Base materials/Ancillary materials
roof window variant covered by the EPD. The declared values The main components of the standard wooden roof window are
in the table relate to the reference product including the variant the glazing unit (made of mainly laminated and tempered
GPL with triple-glazed configuration 66 (GPL --66). For other glass), wooden frames/sashes (made of wood), hinges (made
covered product variants, specific values can be selected at the of steel) and handles/handlebars (made of aluminium). The
bottom of the above-mentioned download page. packaging of the products consists of mostly cardboard along
with paper inserts and galvanised steel.
Constructional data
Name Value Unit
Name Value Unit
Glazing unit (3-layer) 53 %
Reaction to fire C-s1,d2 class
Wooden frame/sash 17 %
Air permeability acc. EN
4 class Steel components (galvanised and stainless) 15 %
12207
Other components (including packaging) 15 %
Resistance to wind load, (for
window width >1140 mm or Recycled content of aluminium 30 %
C3 class
height > 1398 mm no Recycled content of steel 10 %
performance is determined) Recycled content of glass 12 %
4 (toughened) - 13 - 3
The wooden components (sashes, frames) are produced
(heat strengthened) -
Resistance to snow loads mm internally in VELUX facilities, located in Hungary, Poland, and
13 - 6,8 (laminated
Denmark. VELUX receives sawn pine wood (dried) and
float)
processes it (sawing, cutting etc.) into lamellas of different
Water tightness acc. EN
quality. The lamellas are then glued together (lamination) and
12208 unprotected / E900 class
processed into profiles (cutting them into the correct size,
protected
cladding, drilling etc.). For the glazing units, VELUX receives
Impact resistance (for the glazing units components from suppliers and produces the
window width <550 mm or final glazing unit in sites located in Hungary, Denmark, France,
3 class
height <778 mm no and Germany. After their production, the glazing units join the
performance is determined) window assembly process. Finally, the frames/sashes, glazing
Acoustic performance 37 (-2; -4) - unit, and the rest of the components (delivered by suppliers)
Load-bearing capacity of are transported to VELUX assembly sites in Poland, Denmark,
safety devices passed - France and Germany, where they are assembled into the final
window product.
Thermal transmittance, 90
degree installation acc. to 1.0 W/(m2K)
This product/article/at least one partial article contains
EN 10077-1/2
substances listed in the candidate list (date: 23.08.2023)
Solar factor 0.44 -
exceeding 0.1 percentage by mass: NO.
Light transmittance 0.62 -
Reference service life
Product performance data in accordance with DS/EN 14351-
No reference service life (RSL) is defined for the roof windows
1:2006+A2:2016, Windows and doors - Product standard,
because the use stage modules are not included in the EPD.
performance characteristics - Part 1: Windows and external
pedestrian doorsets.
LCA: Calculation rules
Name Value Unit
Declared Unit
Declared unit 1 m2
Multiple product dimensions are represented by this EPD as
specified in the product description. The declared unit is 1 m2 Grammage 47.64 kg/m2
wooden roof window calculated based on the size 1.34 m x Layer thickness (glazing unit) 0.0384 m
1.40 m (UK08), which is the closest available size to the
Data quality and a sensitivity analysis show that the results are
reference window size (1.23 m x 1.48 m based on EN 14351-1)
robust with regard to data quality and appropriateness. There is
with triple glazed window panes. The GPL variant has the
low variability of production processes and product variations
largest weight per m2 in the 2-layer glazing product group.
have a limited influence on the results.
Since the frame/sash construction is alike across all variants in
the product group, the parts that set the variants apart are System boundary
primarily the window-operation components, such as hinges, The type of the EPD is "cradle to gate - with options" including
handles and ventilation flaps. These components are to a high the modules C1-C4 and D. The following life cycle phases were
degree metal-based, and the worst-case product can thus be considered:
identified by the weight of products with similar size and glazing
unit. The heavier the product, the larger the content of metal. Product stage:
Therefore, the GPL variant can be considered more
• A1 - Raw material supply: extraction and processing,
representative as worst-case scenario for the whole roof
production of the pre-products (e.g. laminated glass,
windows group.
sawn pine wood, metal/plastic components, sealants
Declared unit and mass reference etc.) and sales packaging components (e.g.,
cardboard).
• A2 - Transport: Transport of pre-products and packaging
components to the processing or assembly sites, as well
as internal transportation of components between sites.
3 Environmental Product Declaration - VELUX Group - VELUX wooden roof windows (triple glazing configuration)
• A3 - Manufacturing: The wooden frames/sashes and from plastic and wood waste incineration processes and
glazing units are produced internally at VELUX material recycling of metal and glass.
production sites. Subsequently, the final production and
assembly of the windows takes place, which involves For the environmental impact, the use of green electricity was
activities such as shortening of profiles, drilling of holes, calculated taking into account the residual electricity mix for the
clamping and glueing, mounting of gaskets, brackets, remaining electricity. The proportion of the electricity demand
panes etc. covered by green electricity in the total electricity demand is
79.23 %.
End of life stage:
Geographic Representativeness
• C1 - De-construction/demolition: deconstruction of the
Land or region, in which the declared product system is
window with the use of an electric screwdriver and
manufactured, used or handled at the end of the product´s
manual work.
lifespan: Europe
• C2 - Transport: transport of window materials to Material
Recovery Facilities (MRF) and then to incineration,
landfill or recycling facilities. Comparability
• C3 - Waste processing: sorting of waste, recycling
Basically, a comparison or an evaluation of EPD data is only
(metal and glass waste), incineration (plastic and wood
possible if all the data sets to be compared were created
waste) and landfill (metal, glass, wood and plastic
according to EN 15804 and the building context, respectively
waste).
the product-specific characteristics of performance, are taken
• C4 - Disposal: disposal of all materials
into account. Average secondary datasets were retrieved from
the Managed LCA Content (v2021.2) and Ecoinvent (v3.8)
Benefits and loads beyond the system boundaries:
databases.
• D - Reuse, recovery and recycling potential: benefits
LCA: Scenarios and additional technical information
End of life (C1-C4)
Characteristic product properties of biogenic carbon
8.02 kg of wood is used in window's frames/sashes and 0.03 kg Name ValueUnit
of paper inlet is used per declared unit. For the packaging, 3.09 Collected as mixed construction waste 44.48 kg
kg of cardboard and 0.01 kg of paper insert are used per Recycling 16 kg
declared unit.
Energy recovery 10.73 kg
Information on describing the biogenic carbon content at Landfilling 17.76 kg
factory gate
Omitted to atmosphere (Krypton gas in glazing unit) 0.055 kg
Name ValueUnit
kg Reuse, recovery and/or recycling potentials (D), relevant
Biogenic carbon content in product 3.64 C scenario information
Biogenic carbon content in accompanying kg Name Value Unit
2.5
packaging C Wood incinerated 95 %
Note: 1 kg of biogenic carbon is equivalent to 44/12 kg of CO . Plastic incinerated 95 %
2
Paper incinerated 95 %
Metal recycled 95 %
The construction process stage and the use stage modules are Glass recycled 30 %
not declared. However, the quantity of packaging generated in
module A5 is declared as scenario information.
Scenario information for packaging generated in module
A5
Name Value Unit
Cardboard packaging for waste treatment 3.09 kg
Paper packaging for waste treatment 0.01 kg
Steel packaging for waste treatment (galvanised) 0.0032 kg
4 Environmental Product Declaration - VELUX Group - VELUX wooden roof windows (triple glazing configuration)
LCA: Results
DESCRIPTION OF THE SYSTEM BOUNDARY (X = INCLUDED IN LCA; MND = MODULE OR INDICATOR NOT DECLARED; MNR
= MODULE NOT RELEVANT)
Benefits and
Construction loads beyond
Product stage Use stage End of life stage
process stage the system
boundaries
la ire ta m w a Ry lp p u s tro p s n a rT g n iru tc a fu n a M e h t m o rf tro p s n a rTe tis e h t o t e ta g y lb m e s s A e s U e c n a n e tn ia M ria p e R tn e m e c a lp e R tn e m h s ib ru fe R y g re n e la n o ita re p Oe s u re ta w la n o ita re p Oe s u n o itc u rts n o c -e Dn o itilo m e d tro p s n a rT g n is s e c o rp e ts a W la s o p s iD -e s u e R-y re v o c e R-g n ilc y c e Rla itn e to p
A1 A2 A3 A4 A5 B1 B2 B3 B4 B5 B6 B7 C1 C2 C3 C4 D
X X X MND MND MND MND MNR MNR MNR MND MND X X X X X
RESULTS OF THE LCA - ENVIRONMENTAL IMPACT according to EN 15804+A2: 1 m2 VELUX standard wooden roof window
Parameter Unit A1 A2 A3 C1 C2 C3 C4 D
GWP-total kg CO 2 eq 9.69E+01 4.14E-01 2.56E+01 1.97E-03 2.71E+00 1.87E+01 1.83E+00 -3.53E+01
GWP-fossil kg CO 2 eq 1.25E+02 4.11E-01 1.5E+01 1.97E-03 2.66E+00 5.99E+00 2.94E-01 -3.53E+01
GWP-biogenic kg CO 2 eq -2.81E+01 -4.68E-04 1.06E+01 1.1E-06 2.87E-02 1.27E+01 1.53E+00 -4.75E-02
GWP-luluc kg CO 2 eq 8.6E-02 3.29E-03 2.57E-02 3.38E-07 2.2E-02 6.39E-04 7.8E-04 -1.07E-02
ODP kg CFC11 eq 9.72E-07 8.03E-17 1.45E-09 2.22E-17 5.32E-16 -6.84E-09 1.08E-15 -5.18E-14
AP mol H+ eq 5.04E-01 6.54E-04 4.25E-02 3.18E-06 1.62E-02 5.43E-03 2.02E-03 -1.27E-01
EP-freshwater kg P eq 4.67E-03 1.2E-06 1.44E-04 7.92E-10 8E-06 -1.55E-05 3.41E-06 -1.87E-05
EP-marine kg N eq 1.05E-01 2.21E-04 1.67E-02 8.43E-07 7.92E-03 2.33E-03 5.52E-04 -2.65E-02
EP-terrestrial mol N eq 1.18E+00 2.55E-03 1.73E-01 9.03E-06 8.77E-02 2.89E-02 5.92E-03 -2.93E-01
kg NMVOC
POCP 2.97E-01 6.02E-04 3.97E-02 2.39E-06 1.47E-02 6.15E-03 1.88E-03 -7.21E-02
eq
ADPE kg Sb eq 2.12E-03 3.59E-08 1.4E-05 2.44E-10 2.39E-07 -7.53E-08 2.66E-08 -7.15E-06
ADPF MJ 1.7E+03 5.46E+00 2.25E+02 4.08E-02 3.59E+01 5.6E+00 3.93E+00 -4.23E+02
m3 world eq
WDP 8.55E+00 3.75E-03 6.94E-01 1.58E-04 2.5E-02 2.08E+00 3.04E-02 -1.95E+00
deprived
GWP = Global warming potential; ODP = Depletion potential of the stratospheric ozone layer; AP = Acidification potential of land and water; EP =
Eutrophication potential; POCP = Formation potential of tropospheric ozone photochemical oxidants; ADPE = Abiotic depletion potential for non-fossil
resources; ADPF = Abiotic depletion potential for fossil resources; WDP = Water (user) deprivation potential)
RESULTS OF THE LCA - INDICATORS TO DESCRIBE RESOURCE USE according to EN 15804+A2: 1 m2 VELUX standard
wooden roof window
Parameter Unit A1 A2 A3 C1 C2 C3 C4 D
PERE MJ 5.51E+02 3.09E-01 4.3E+02 4.21E-03 2.06E+00 1.04E+00 4.95E-01 -7.37E+01
PERM MJ 8.34E-02 0 0 0 0 0 0 0
PERT MJ 5.52E+02 3.09E-01 4.3E+02 4.21E-03 2.06E+00 1.04E+00 4.95E-01 -7.37E+01
PENRE MJ 1.58E+03 5.48E+00 2.26E+02 4.09E-02 3.6E+01 1.02E+02 3.93E+00 -4.24E+02
PENRM MJ 1.32E+02 0 -5.09E-01 0 0 -9.62E+01 0 0
PENRT MJ 1.71E+03 5.48E+00 2.25E+02 4.09E-02 3.6E+01 5.61E+00 3.93E+00 -4.24E+02
SM kg 3.82E+00 0 0 0 0 0 0 0
RSF MJ 0 0 0 0 0 0 0 0
NRSF MJ 0 0 0 0 0 0 0 0
FW m3 5.5E-01 3.54E-04 6.69E-02 9.2E-06 2.36E-03 4.91E-02 9.22E-04 -1.78E-01
PERE = Use of renewable primary energy excluding renewable primary energy resources used as raw materials; PERM = Use of renewable primary
energy resources used as raw materials; PERT = Total use of renewable primary energy resources; PENRE = Use of non-renewable primary energy
excluding non-renewable primary energy resources used as raw materials; PENRM = Use of non-renewable primary energy resources used as raw
materials; PENRT = Total use of non-renewable primary energy resources; SM = Use of secondary material; RSF = Use of renewable secondary fuels;
NRSF = Use of non-renewable secondary fuels; FW = Use of net fresh water
RESULTS OF THE LCA – WASTE CATEGORIES AND OUTPUT FLOWS according to EN 15804+A2:
1 m2 VELUX standard wooden roof window
Parameter Unit A1 A2 A3 C1 C2 C3 C4 D
HWD kg 3.25E-03 2.84E-10 1.26E-06 4.91E-12 1.9E-09 1.08E-09 4.58E-10 -4.07E-08
NHWD kg 7.71E+00 8.54E-04 3.47E-01 7.68E-06 5.65E-03 9.62E-01 1.72E+01 -3.16E+00
RWD kg 4.13E-02 9.87E-06 1.09E-02 6.61E-06 6.53E-05 2.6E-04 4.18E-05 -1.65E-02
CRU kg 0 0 0 0 0 0 0 0
MFR kg 1.77E-02 0 1.66E+01 0 0 1.6E+01 0 0
MER kg 0 0 0 0 0 1.04E+01 0 0
EEE MJ 3.51E-02 0 0 0 0 3.28E+01 0 0
EET MJ 5.13E-02 0 0 0 0 5.98E+01 0 0
5 Environmental Product Declaration - VELUX Group - VELUX wooden roof windows (triple glazing configuration)
HWD = Hazardous waste disposed; NHWD = Non-hazardous waste disposed; RWD = Radioactive waste disposed; CRU = Components for re-use;
MFR = Materials for recycling; MER = Materials for energy recovery; EEE = Exported electrical energy; EET = Exported thermal energy
RESULTS OF THE LCA – additional impact categories according to EN 15804+A2-optional:
1 m2 VELUX standard wooden roof window
Parameter Unit A1 A2 A3 C1 C2 C3 C4 D
Disease
PM 8.56E-06 7.85E-09 4.18E-07 2.9E-11 7.01E-08 3.34E-08 2.45E-08 -1.25E-06
incidence
IR kBq U235 eq 8.41E+00 1.44E-03 1.51E+00 9.66E-04 9.55E-03 3.08E-02 4.64E-03 -3.1E+00
ETP-fw CTUe 1.99E+03 4.05E+00 6.36E+01 1.25E-02 2.66E+01 2.72E+00 2.54E+00 -1.81E+02
HTP-c CTUh 6.52E-07 8.18E-11 9.33E-09 2.09E-13 5.38E-10 1.4E-10 3.07E-10 -2.85E-08
HTP-nc CTUh 2.02E-06 4.24E-09 2.19E-07 1.16E-11 3.3E-08 9.15E-09 3.43E-08 -2.79E-07
SQP SQP 5.19E+03 1.84E+00 3.76E+02 3.39E-03 1.23E+01 5.58E-01 7.2E-01 -2.09E+01
PM = Potential incidence of disease due to PM emissions; IR = Potential Human exposure efficiency relative to U235; ETP-fw = Potential comparative
Toxic Unit for ecosystems; HTP-c = Potential comparative Toxic Unit for humans (cancerogenic); HTP-nc = Potential comparative Toxic Unit for humans
(not cancerogenic); SQP = Potential soil quality index
Disclaimer 1 – for the indicator 'Potential Human exposure efficiency relative to U235'. This impact category deals mainly with the
eventual impact of low-dose ionizing radiation on human health of the nuclear fuel cycle. It does not consider effects due to possible
nuclear accidents, occupational exposure or radioactive waste disposal in underground facilities. Potential ionizing radiation from the
soil, radon and from some construction materials is also not measured by this indicator.
Disclaimer 2 – for the indicators 'abiotic depletion potential for non-fossil resources', 'abiotic depletion potential for fossil resources',
'water (user) deprivation potential, deprivation-weighted water consumption', 'potential comparative toxic unit for ecosystems', 'potential
comparative toxic unit for humans – cancerogenic', 'Potential comparative toxic unit for humans - not cancerogenic', 'potential soil
quality index'. The results of this environmental impact indicator shall be used with care as the uncertainties on these results are high
as there is limited experience with the indicator.
The results show that module A1 has the highest impact across all environmental impact indicators (except GWP – biogenic). Module
A3 has the second highest impact in most impact indicators due to the energy consumption and the use of residual electricity grid mix.
All main components in the windows contribute significantly to some of the environmental indicators, except for wood, which is only
significant for the GWP-luluc and WDP indicators. The glass in the glazing units has the highest contribution in most impact categories
among all material types. The galvanized steel components contribute significantly to the results due to their high weight contribution to
the product. The aluminium components are also significant for the WDP indicator, although the weight of the aluminium components is
notably lower in comparison with the galvanized steel components. This is most likely due to the relatively high energy and water
consumption in the production of aluminium. It is noted that the production activities at VELUX contribute significantly to the GWP-fossil
and ADPF impact indicators therefore, the actual impact contribution of the final wooden components is higher than the impact of
upstream processed wood production.
References
IBU PCR Part A
IBU PCR Part A: Institut Bauen und Umwelt e.V., Product ISO 14025
Category Rules for Building-Related Products and Services. DIN EN ISO 14025:2011-10, Environmental labels and
Calculation Rules for the Life Cycle Assessment and declarations - Type III environmental declarations - Principles
Requirements on the Project Report according to EN and procedures.
15804+A2:2019, version 1.3.
EN 14351-1
IBU PCR Part B EN 14351-1:2006+A2:2016, Windows and doors - Product
IBU PCR Part B: Institut Bauen und Umwelt e.V., Requirements standard, performance characteristics - Part 1: Windows and
on the EPD for Windows and doors, version 1.4: 2021. external pedestrian doorsets.
IBU 2021 EN 15804
IBU 2021 Institut Bauen und Umwelt e.V.: General Instructions EN 15804:2012+A2:2019+AC:2021, Sustainability of
for the EPD programme of Institut Bauen und Umwelt e.V. construction works — Environmental Product Declarations —
Version 2.0, Berlin: Institut Bauen und Umwelt e.V., 2021. Core rules for the product category of construction products.
www.ibu-epd.com.
EN 17213
EN 12207 EN 17213:2020, Windows and doors – Environmental Product
EN 12207:2016 Windows and doors - Air permeability - Declarations – Product category rules for windows and
Classification pedestrian doorsets.
EN 12208 Regulation (EU) No 305/2011
EN 12208:2000 Windows and doors. Regulation (EU) No 305/2011 of the European Parliament and
Watertightness.Classification is classified in these ICS of the Council of 9 March 2011 laying down harmonised
categories: 91.060.50Doors and windows conditions for the marketing of construction products
andrepealing Council Directive 89/106/EEC
EN 13501-1
EN 13501-1 EN13501-1, 2018: Fire classification of Candidate list
construction products and building elements - Part 1: ECHA Candidate list of substances of very high concern, status
Classification using data from reaction to fire tests. 23.08.2023
6 Environmental Product Declaration - VELUX Group - VELUX wooden roof windows (triple glazing configuration)
Numerical method for frames.
ISO 10077-1
ISO 10077-1:2017, Thermal performance of windows, doors LCA for Experts (GaBi) LCA software, Managed LCA
and shutters - Calculation of thermal transmittance - Part 1: Content and Ecoinvent databases
General. The LCA modelling software is LCA for Experts program
version 10.7.1 with corresponding databases from Sphera
ISO 10077-2 Solutions GmbH (Managed LCA Content) and Ecoinvent.
ISO 10077-2:2017, Thermal performance of windows, doors Documentation hyperlink www.gabisoftware. com/support/gabi.
and shutters - Calculation of thermal transmittance - Part 2:
7 Environmental Product Declaration - VELUX Group - VELUX wooden roof windows (triple glazing configuration)
Publisher
Institut Bauen und Umwelt e.V. +49 (0)30 3087748- 0
Hegelplatz 1 info@ibu-epd.com
10117 Berlin www.ibu-epd.com
Germany
Programme holder
Institut Bauen und Umwelt e.V. +49 (0)30 3087748- 0
Hegelplatz 1 info@ibu-epd.com
10117 Berlin www.ibu-epd.com
Germany
Author of the Life Cycle Assessment
FORCE Technology +4543250856
Park Alle 345 chme@forcetechnology.com
2605 Brøndby www.forcetechnology.com
Denmark
Owner of the Declaration
VELUX Group +4545164871
Ådalsvej 99 birthe.kjeldsen@velux.com
2970 Hørsholm www.velux.com
Denmark
8 Environmental Product Declaration - VELUX Group - VELUX wooden roof windows (triple glazing configuration)
