ENVIRONMENTAL PRODUCT DECLARATION
as per ISO 14025 and EN 15804+A2
Owner of the Declaration VELUX Group
Publisher Institut Bauen und Umwelt e.V. (IBU)
Programme holder Institut Bauen und Umwelt e.V. (IBU)
Declaration number EPD-VEL-20230508-IBA1-EN
Issue date 29.01.2024
Valid to 28.01.2029
VELUX glass architecture made from a BA 5/6 glazing system and
VENTRIA 3 system sashes
VELUX Group
www.ibu-epd.com | https://epd-online.com
1. General Information
VELUX Group VELUX glass architecture made from a BA 5/6
glazing system and VENTRIA 3 system sashes
Programme holder Owner of the declaration
IBU – Institut Bauen und Umwelt e.V. VELUX Group
Hegelplatz 1 Ådalsvej 99
10117 Berlin 2970 Hørsholm
Germany Denmark
Declaration number Declared product / declared unit
EPD-VEL-20230508-IBA1-EN 1 m2 of VELUX glass architecture made from a BA 5/6 glazing system and
VENTRIA 3 system sashes produced by VELUX group; the EPD covers
versions made from 2-layered insulation glass as well as 3-layered
insulation glass.
This declaration is based on the product category rules: Scope:
Windows and doors , 01.08.2021 The LCA represents 100% of the production volume of VELUX glass
(PCR checked and approved by the SVR) architecture made from a BA 5/6 glazing system and VENTRIA 3 system
sashes, produced by Velux in Voerde, Germany.
The owner of the declaration shall be liable for the underlying information
Issue date and evidence; the IBU shall not be liable with respect to manufacturer
information, life cycle assessment data and evidences.
29.01.2024
The EPD was created according to the specifications of EN 15804+A2. In
the following, the standard will be simplified as EN 15804.
Valid to
28.01.2029 Verification
The standard EN 15804 serves as the core PCR
Independent verification of the declaration and data according to ISO
14025:2011
internally X externally
Dipl.-Ing. Hans Peters
(Chairman of Institut Bauen und Umwelt e.V.)
Florian Pronold Dr.-Ing. Nikolay Minkov,
(Managing Director Institut Bauen und Umwelt e.V.) (Independent verifier)
1 Environmental Product Declaration - VELUX Group - VELUX glass architecture made from a BA 5/6 glazing system and VENTRIA 3 system sashes
2. Product
2.1 Product description/Product definition
This EPD for a glass roof construction includes the following VENTRIA 3 system sash
products:
• BA 5/6 glazing system According to EN 14351-1:
• VENTRIA 3 system sashes • resistance to wind load according to EN 12210 - class
The aluminium profiles are powder coated and fixed to the C5/B5
target object using screws. • water tightness according to EN 12208 - up to class
E1950
ET-BA 5/6 glazing system • air permeability according to EN 12207 - class 4
• individually plannable mullion-transom system for glass • thermal insulation Uw value = 1.2 W/m²K (reference
constructions in roofs and walls value)
• can be designed as a certified passive house Performance data of the product in accordance with the
component declaration of performance with respect to its essential
• profile system: characteristics according to:
- construction made of torsion-resistant aluminium • EN 12101-2, Smoke and heat control systems - Part 2:
- water and condensate drainage via two drainage Natural smoke and heat exhaust ventilators
levels • EN 14351-1,Windows and doors - Product standard,
- flexible polygonal shape from 2° to 90 performance characteristics - Part 1: Windows and
- clamp connection approved by the building authorities external pedestrian doorsets.
with building authority approval No. Z-14.4-486 • EN 13830, Curtain walling - Product standard
- visible elements of the supporting structure • building authority approval No. Z-14.4-486
(aluminium) and roof panels with RAL coating possible
• building connection: mounting on concrete, wooden 2.4 Delivery status
upstand or on sheet steel frame possible The glass elements are avilable in sizes ranging from 0.2 m2 up
VENTRIA 3 system sashes to 4.5 m2, which can be combined to any total glass area as
• system sash with flat overall height for daily ventilation needed.
and for qualified smoke and heat ventilation
2.5 Base materials/Ancillary materials
• welded corner joints for permanent dimensional stability
• stepless installation in roof pitches from 0° to 90 Name Value Unit
66 % to 69
glass -
For the placing on the market of the product in the European %
Union/European Free Trade Association (EU/EFTA) (with the 12 % to 15
aluminium -
exception of Switzerland) Regulation (EU) No. 305/2011 (CPR) %
applies. The product needs a declaration of performance taking
16 % to 17
into consideration: steel, low-alloyed -
%
• EN 12101-2,, Smoke and heat control systems - Part 2: ethylene propylene diene monomer rubber
Natural smoke and heat exhaust ventilators (EPDM) 1 % -
• EN 14351-1,Windows and doors - Product standard,
others 1 % to 2 % -
performance characteristics - Part 1: Windows and
external pedestrian doorsets.
• EN 13830, Curtain walling - Product standard 1. This product/article/at least one partial article contains
• general building authority approval No. Z-14.4-486 substances listed in the ECHA candidate list (date: 15.08.2023)
and the CE-marking. exceeding 0.1 percentage by mass: no.
2.2 Application 2. This product/article/at least one partial article contains other
In addition to its actual function as a roof, the glass roof carcinogenic, mutagenic or reprotoxic (CMR) substances in
construction also serves to increase daylight incidence and categories 1A or 1B which are not on the ECHA candidate list,
natural ventilation. exceeding 0.1 percentage by mass: not investigated with
suppliers.
2.3 Technical Data
3. Biocide products were added to this construction product or it
has been treated with biocide products (this then concerns a
BA 5/6 glazing system treated product as defined by the (EU) Ordinance on Biocide
Products No. 528/2012): no.
In accordance with EN 13830:
2.6 Manufacture
• water tightness - class RE 1950
After completion of the technical elaborations of the glass
• air permeability - class AE
architecture, the aluminium profiles are cut to size, machined
• resistance to wind load
and, if necessary, welded. After machining in the raw state, the
• 2.0 kN/m² (permissible load)
profiles are powder-coated. The coated profiles are then
• 3.0 kN/m² (increased load)
assembled ready for the construction site and packed on
• general building authority approval (clamp connection)
pallets for transport.
All declared structural-physical properties have been tested and
In order to guarantee the quality assurance of the product,
certified.
VELUX operates a quality management system according to
ISO 9001.
2 Environmental Product Declaration - VELUX Group - VELUX glass architecture made from a BA 5/6 glazing system and VENTRIA 3 system sashes
properties (tested individually):
2.7 Environment and health during manufacturing Aluminium, steel, stainless steel: no fire test
The factory is ISO 14001 and ISO 45001 certified. Glass: no fire test
Gasket EPDM: class E , EN 13501
2.8 Product processing/Installation
Styrodur: class E, EN 13501
The mullion and transom profiles (BA 5/6 glazing system) are Polyamid: class E, EN 13501
screwed together and fixed to the substructure. The type of EPDM foil: class B, DIN 4102-1
fastening depends on the substructure. Alufixband, Butyltape: class B2, DIN 4102-1
After completion of the aluminium construction, glazing is Glazing pad: class B2, DIN 4102-1
carried out. The glass panes are secured and sealed with cover
strips. A VENTRIA 3 system sash is installed in the same way
as a pane of glass. Afterwards, the wall connections and the Water
construction of the eaves and ridge area take place. In the event of unforeseen exposure to water (flood), electrical
components need be replaced; no adverse effects on human
2.9 Packaging
health or the environment are to be expected.
The packaging usually consists of:
• polyethylene film Mechanical destruction
• wooden laths In the event of unforeseen mechanical destruction, VELUX
The use of other packaging materials is possible, but glass architecture must be replaced; apart from potential
insignificant in terms of quantity. injuries from glass cullet, no adverse effects on human health
or the environment are to be expected.
The packaging materials can be recycled if separated by type;
alternatively, they can be incinerated. 2.14 Re-use phase
VELUX glass architecture can be dismantled manually without
2.10 Condition of use any problems. The metal parts are usually recycled, and the
The material composition of VELUX glass architecture does not plastic parts are sent for thermal recycling for energy recovery.
change over their service life. Flat glass can be recycled.
2.11 Environment and health during use 2.15 Disposal
VELUX glass architecture does not contain any pollutants that VELUX glass architecture is mostly inert and can be disposed
could be released during use. of in an appropriate landfill. However, due to the value of the
materials or the carbon content of the plastic parts, recycling or
Environmental protection: According to current knowledge, energy recovery is preferable and common.
hazards to water, air and soil cannot arise when the products
are used as intended. Waste code according to the European Waste List (Regulation
on the European Waste List):
Health protection: According to current knowledge, no health
hazards or impairments are to be expected. 17 02 02 glass
17 02 03 plastics
2.12 Reference service life
17 04 14 mixed metals
It is not possible to calculate the reference service life
according to ISO 15686. The service life based on a 2.16 Further information
manufacturer's declaration is 50 years. The corresponding Further documentation on the products, technical data sheets,
utilization scenario is declared in chapter 4. BIM files, etc. can be found at:
2.13 Extraordinary effects
www.velux.com
Fire
The components of the glass architecture have the following
3. LCA: Calculation rules
The representative glass architecture system consists of a total
3.1 Declared Unit of 1097 m² roof area including 32 VENTRIA 3 system sashes
1 m2 of VELUX glass architecture made from a BA 5/6 glazing (max. area 4 m2/VENTRIA 3) resulting in:
system and VENTRIA 3 system wings produced by VELUX
group; the EPD covers versions made from 2-layered insulation Rooflight 1069 m²
glass as well as 3-layered insulation glass. Eave and top 28.5 m²
Declared unit and mass reference (with 3-layered Total 1097 m²
insulation glass))
3.2 System boundary
Name Value Unit
Type of the EPD: "cradle to gate with options, with modules
Declared unit 1 m2 C1–C4, and module D (A1–A3, C, D and additional modules.
Grammage 89.3 kg/m2 The additional modules may be modules A4 and/or A5 and/or
B1–B7)". In this EPD, modules A4, A5, B2 and B6 are declared
A representative glass building project from 2016 was scaled to
as additional modules.
the declared unit, as there is no typical functional unit due to
the high number of variants. Where possible, the worst-case
The production of VELUX glass architecture (modules A1-A3)
approach was followed. This means that the worst values or
includes raw material extraction, energy generation, waste
assumptions were used in this analysis to determine the
treatment and all transports up to the factory gate. In
material and energy flows; e.g., the version with 3-layered
accordance with COUNCIL REGULATION (EU) No 333/2011,
insulation glass is declared.
3 Environmental Product Declaration - VELUX Group - VELUX glass architecture made from a BA 5/6 glazing system and VENTRIA 3 system sashes
secondary metals are modelled as part of the product system
from the moment they are available as unmixed scrap. Smoke and heat extraction systems or ventilation systems are
Waste or secondary fuels are not used for production. enabled by pneumatic or electrically operated drive systems to
remove smoke and/or heat from buildings or to ensure
Module A4 describes the transport from the production site to ventilation in module B6. The inputs and outputs from the
the construction. A transport by lorry over an average transport operation of electrical control centres and pneumatic
distance of 400 km has been assumed based on the maximum valves/alarm stations are not taken into account.
distances to customers in Germany.
Module B7 is not relevant for the declared products. The
For the installation of the glass elements in module A5, a crane indicator values of Module B7 are thus 0 nd not declared in the
and a lifting platform are required. EPD.
The mullion and transom profiles (BA 5/6 glazing system) are
screwed together and fixed to the substructure. For the de-installation of the glass elements in module C1, a
Waste is collected separately and taken to a recycling plant. crane and a lifting platform are required. The mullion and
The main waste produced here is wood waste and plastic transom profiles (VELUX BA 5/6 glazing system) are un-
packaging, which is recycled for energy recovery. screwed together and disassembled from the substructure.
The products are assumed to have no direct emissions during
the use phase (module B1). The indicator values of Module B1 Given the complexity of the inventoried products, a mixed end-
are thus 0 and not declared in the EPD. of-life scenario is modelled, allowing the different materials to
follow their most likely path.
Module B2 includes the cleaning, the annual functionality test
and the replacement of components over the service life. Metals and flat glass are recycled; it is assumed that these
fractions reach end-of-waste state after having been sorted and
Cleaning transported to a recycler. Plastics are incinerated (also due to
The glass roofs are cleaned manually every 2 months. The the very limited data availability on plastics recycling and its
amount of cleaning water is taken into account. Due to the low benefits). On average, an average transport distance of 75 km
concentration of surfactants in the cleaning water, this is not has been assumed in module C2 with an average lorry for the
taken into account (cut-off criterion). No other auxiliary transport of the wastes to an incineration plant or to a recycling
substances are used. The wastewater is fed into a municipal facility.
sewage treatment plant.
A glass construction can either consist of glass elements that The disassembled product is shredded and the materials are
can be walked on or there is an access system to carry out the sorted in module C3. The recovered material leaves the
cleaning process. In this study, an access system is seen as a product system as 'materials for recycling'. The net amounts of
component of the building and is not included in the the metals leaving the product system are considered as 'use of
calculations. secondary material' in Module D.
Current care and maintenance instructions VELUX glass
structures are provided for each building project. In module C4, plastic parts are treated in a waste incineration
plant with an efficiency R1 < 0.6 (according to CEWEP Energy
Functionality test Report III); The recovered energy is reported as 'exported
An annual functionality check of the window elements is carried energy' and considered in Module D.
out. This consists of a visual inspection and occasional
lubrication and greasing of the moving parts. Module D contains the benefits and loads beyond the system
In addition, maintenance required by law for smoke and heat boundary related to the recycling of metals and glass, which
extraction systems is carried out at regular intervals of at least result from the treatment of recycled materials from the point of
once a year. end-of-waste status to the point of substitution (as loads) and
Auxiliary materials and waste as well as transport routes during the substitution of primary resources (as benefits).
maintenance are negligible and are not considered in this study. It also includes the benefits and loads related to the energy
The closing cycles are attributed to normal operation. recovery from plastic wastes in a municipal waste incineration
plant as modelled in Modules A5 and C4.
Replacement of components Only net flows leaving the product system are considered in
If the glass architecture is used as intended, the following module D.
maintenance measures are to be expected for the VENTRIA 3
system over a service life of 50 years: 3.3 Estimates and assumptions
No further assumptions and estimates relevant to the result had
• one-time replacement of the fittings (stainless steel
to be made beyond the points made in chapter 3 and chapter 4.
screws and plates)
• one-time replacement of the seals (EPDM) 3.4 Cut-off criteria
• one-time replacement of the drive system (motor and its
No data available from the company survey was neglected.
console)
These include, among other things, material use, energy
Auxiliary materials, waste materials, material losses as well as
demand (heat, electricity), packaging materials of raw materials
transport routes during the repair are negligible. The
(insofar as they are generated as waste) and product
consumption of fresh water for cleaning purposes and the
packaging, consumables in production, waste treatment and
energy for screwing processes are neglected in this one-time
the transport of all inputs and outputs.
repair measure.
With this approach, mass and energy flows below 1 % were
Recovered metals are recycled, the seals are incinerated in a
also accounted for. No processes were neglected that would
municipal waste incineration plant with energy recovery.
have been known to the project managers and would have
contributed significantly to the indicators of the impact
Modules B3 to B5 are not relevant for the declared products.
assessment.
The indicator values of Modules B3 to B5 are thus 0 and not
declared in the EPD.
4 Environmental Product Declaration - VELUX Group - VELUX glass architecture made from a BA 5/6 glazing system and VENTRIA 3 system sashes
metals, notably aluminium, is considered a secondary material
3.5 Background data with no economic value (so no burdens allocated) and
Ecoinvent v3.9.1 (2022) with the system model 'allocation – cut- considered in the quantification of net flows leaving the product
off by classification – unit processes' is used as the background system. This approach is chosen to ensure a coherent
database. quantification of net flows entering module D.
3.6 Data quality
Biogenic carbon is allocated based on physical flows
The foreground data are based on extensive and detailed data regardless of the allocation procedure chosen for the process.
collection at the production site. The foreground data could be The biogenic carbon content of wood products entering or
fully linked with corresponding data records from the leaving the product system is quantified (manually) as part of
background database ecoinvent v3.9.1 with the system model the GWP in conformity with EN 16485.
"allocation – cut-off by classification – unit processes".
No processes were modelled as part of the foreground model
The background data was updated in 2022. Thus, the quality of that would have required an allocation of multi-input processes.
the foreground and background data can be rated as very Background datasets on municipal waste incineration plants
good. were taken from ecoinvent without any modification.
3.7 Period under review
Allocation of reuse, recycling and recovery was avoided by the
The LCA data represents the production conditions for the year
cut-off approach in the foreground model in line with EN 15804.
2022.
3.10 Comparability
3.8 Geographic Representativeness
Basically, a comparison or an evaluation of EPD data is only
Land or region, in which the declared product system is
possible if all the data sets to be compared were created
manufactured, used or handled at the end of the product´s
according to EN 15804 and the building context, respectively
lifespan: Germany
the product-specific characteristics of performance, are taken
into account.
3.9 Allocation Ecoinvent v3.9.1 (2022) with the system model 'allocation – cut-
off by classification – unit processes' is used as the background
No co-products are generated during the production of the
database.
VELUX products. Sorted production scrap of the different
4. LCA: Scenarios and additional technical information
Reference service life
Characteristic product properties of biogenic carbon
Note: 1 kg of biogenic carbon is equivalent to 44/12 kg of CO .
2
Information on describing the biogenic carbon content at
factory gate
Name ValueUnit
kg
Biogenic carbon content in product -
C
Biogenic carbon content in accompanying kg
0.104
packaging C
Module A4
A transport by lorry over an average transport distance of 400
km has been assumed based on the maximum distances to
customers in Germany
Module A5
For the installation of the glass elements, a crane and a lifting
platform are required, which lift the product to be installed to an
assumed height of 20 m.
The mullion and transom profiles (VELUX BA 5/6 glazing
system) are screwed together and fixed to the substructure.
The cordless screwdriver can process 170 screws with one
battery charge (0.0234 kWh).
The packaging material (5 kg of plastics, 250 kg of wood) is
assumed to be transported 50 km with an average lorry to an
incineration plant with an efficiency R1 < 0.6 (according to
CEWEP Energy Report III); according to the same source, an
efficiency of 31.0 % is assumed for the production of heat and
18.0 % for the production of electricity (always referring to the
lower heating value of the waste). The recovered energy is
declared as exported energy.
5 Environmental Product Declaration - VELUX Group - VELUX glass architecture made from a BA 5/6 glazing system and VENTRIA 3 system sashes
Name Value Unit Auxiliary materials, waste materials, material losses as well as
transport routes during the repair are negligible. The
Life Span according to
50 a consumption of fresh water for cleaning purposes and the
the manufacturer
energy for screwing processes are neglected in this one-time
The product has passed internal
Declared product repair measure.
quality controls and complies
properties (at the gate) - Recovered metals are recycled, the seals are incinerated in a
with product standard for CE
and finishes municipal waste incineration plant with energy recovery (for its
marking
efficiencies and transport distances, see above)
Design application
parameters (if instructed
Module B6
by the manufacturer), Installation according to
The energy consumption in the period of use (B6) relates
including the references assembly instructions and state -
exclusively to the pneumatic or electric drives and is included in
to the appropriate of the art.
the sample EPD "Electric drives and pneumatic cylinders" from
practices and application
ift Rosenheim (declaration number: M-EPD-AZR-002). This
codes
EPD has 1 watt or 1 mm cylinder diameter as a reference
An assumed quality of value. The cylinders used have a diameter of 63 mm and were
work, when installed in installed a total of 32 times on a roof area of 1097 m².
Carried out in accordance with
accordance with the - Accordingly, the values for electricity consumption of the
the manufacturer's instructions.
manufacturer’s sample EPD were multiplied by the factor 63￿32/1097 = 1.838
instructions
Outdoor environment, Module C1
The declared products are
(for outdoor For the de-installation of the glass elements, a crane and a
intended for installation outside
applications), e.g. lifting platform are required, which lift down the product to be
the building: They are therefore
weathering, pollutants, - installed from an assumed height of 20 m.
designed to withstand outdoor
UV and wind exposure, The mullion and transom profiles (VELUX BA 5/6 glazing
conditions throughout their
building orientation, system) are un-screwed together and disassembled from the
service life.
shading, temperature substructure. The cordless screwdriver can process 170 screws
Indoor environment (for with one battery charge (0.0234 kWh).
The declared products are not
indoor applications), e.g.
temperature, moisture, intended for installation inside a - Module C2
chemical exposure building. Metals and flat glass are recycled; it is assumed that these
fractions reach end-of-waste state after having been sorted and
Usage conditions, e.g. Standard use in any type of
transported to a recycler. Plastics are incinerated (also due to
frequency of use, building, i.e., opening/closing as -
the very limited available on plastics recycling and its benefits).
mechanical exposure often as necessary.
On average, an average transport distance of 75 km has been
The declared products are
assumed with an average lorry for the transport of the wastes to
designed for a reference service
Maintenance e.g. an incineration plant or to a recycling facility.
life of 50 years, with the
required frequency, type
sealings, fittings and the motor
and quality and - Module C3
replaced every 25 years. They
replacement of A consumption of 0.03 kWh/kg of electricity for shredding and
are maintained by cleaning
components sorting and 0.437 MJ/kg of diesel fuel for internal logistics are
water at the discretion of the
taken into account to disassemble the product. The recovered
building occupants.
material leaves the product system as 'materials for recycling'.
Module B1 The net amounts of the metals leaving the product system are
The products are assumed to have no direct emissions during considered as 'use of secondary material' in Module D.
the use phase. The indicator values of Module B1 are thus 0
and not declared in this EPD. Module C4
As stated above, it is assumed that 100 % of the plastic parts
Module B2 are treated in a waste incineration plant with an efficiency R1
The glass roofs are cleaned manually every 2 months. The < 0.6 (according to CEWEP Energy Report III); according to the
water requirement is taken into account. Due to the low same source, an efficiency of 31.0 % is assumed for the
concentration of surfactants in the cleaning water, this is not production of heat and 18.0 % for the production of electricity
taken into account (cut-off criterion). No other auxiliary (always referring to the lower heating value of the waste). The
substances are used. The wastewater is fed into a municipal recovered energy is reported as 'exported energy' and
sewage treatment plant. The associated water use per m2 has considered in Module D.
been taken from the previous project report (Brands & Values
2017). Module D
Module D contains the benefits and loads beyond the system
The following maintenance measures have been inventoried for boundary related to the recycling of metals and glass, which
the VENTRIA 3 system over a service life of 50 years: result from the treatment of recycled materials from the point of
end-of-waste status to the point of substitution (as loads) and
• one-time replacement of the fittings (stainless steel the substitution of primary resources (as benefits).
screws and plates It also includes the benefits and loads related to the energy
• one-time replacement of the seals (EPDM) recovery from plastic wastes in a MWIP as modelled in
• one-time replacement of the drive system (motor and its Modules A5 and C4.
console) Only net flows leaving the product system are considered in
module D.
6 Environmental Product Declaration - VELUX Group - VELUX glass architecture made from a BA 5/6 glazing system and VENTRIA 3 system sashes
5. LCA: Results
The set of characterisation factors EF 3.1 has been used.
DESCRIPTION OF THE SYSTEM BOUNDARY (X = INCLUDED IN LCA; MND = MODULE OR INDICATOR NOT DECLARED; MNR
= MODULE NOT RELEVANT)
Benefits and
Construction loads beyond
Product stage Use stage End of life stage
process stage the system
boundaries
la ire ta m w a Ry lp p u s tro p s n a rT g n iru tc a fu n a M e h t m o rf tro p s n a rTe tis e h t o t e ta g y lb m e s s A e s U e c n a n e tn ia M ria p e R tn e m e c a lp e R tn e m h s ib ru fe R y g re n e la n o ita re p Oe s u re ta w la n o ita re p Oe s u n o itc u rts n o c -e Dn o itilo m e d tro p s n a rT g n is s e c o rp e ts a W la s o p s iD -e s u e R-y re v o c e R-g n ilc y c e Rla itn e to p
A1 A2 A3 A4 A5 B1 B2 B3 B4 B5 B6 B7 C1 C2 C3 C4 D
X X X X X MND X MNR MNR MNR X MND X X X X X
RESULTS OF THE LCA - ENVIRONMENTAL IMPACT according to EN 15804+A2: 1 m² of the VELUX BA 5/6 glazing system with
VENTRIA 3 system sashes
Parameter Unit A1-A3 A4 A5 B2 B6 C1 C2 C3 C4 D
GWP-total kg CO 2 eq 3.33E+02 5.45E+00 3.73E-01 7.67E+00 1.89E-01 0 1.02E+00 5.84E+00 4.3E+00 -1.67E+02
GWP-fossil kg CO 2 eq 3.32E+02 5.44E+00 3.99E-02 7.65E+00 1.89E-01 0 1.02E+00 5.84E+00 4.3E+00 -1.67E+02
GWP-
biogenic kg CO 2 eq 4.44E-01 4.98E-03 3.33E-01 1.48E-02 -3.15E-04 0 9.31E-04 -2.05E-03 3.95E-04 2.38E-01
GWP-luluc kg CO 2 eq 6.11E-01 2.61E-03 1.78E-05 7.18E-03 2.3E-05 0 4.89E-04 6.47E-04 1.94E-05 -5.12E-01
ODP kg CFC11 eq 6.27E-06 1.16E-07 5.72E-10 9.01E-08 2.09E-09 0 2.18E-08 8.19E-08 3.78E-09 -1.74E-06
AP mol H+ eq 2.21E+00 2.48E-02 1.72E-04 3.24E-02 4.96E-04 0 4.63E-03 4.01E-02 5.73E-04 -1.05E+00
EP-
kg P eq 1.11E-02 4.36E-05 7.78E-07 2.18E-04 9.19E-06 0 8.15E-06 1.04E-04 7.54E-07 -6.49E-03
freshwater
EP-marine kg N eq 3.67E-01 9.75E-03 5.37E-05 5.06E-03 9.66E-05 0 1.82E-03 1.75E-02 2.34E-04 -1.57E-01
EP-terrestrial mol N eq 4.18E+00 1.05E-01 6.05E-04 5.67E-02 1.12E-03 0 1.97E-02 1.91E-01 2.6E-03 -1.87E+00
kg NMVOC
POCP 1.33E+00 3.68E-02 2.11E-04 2.45E-02 3.41E-04 0 6.88E-03 5.67E-02 6.82E-04 -5.81E-01
eq
ADPE kg Sb eq 1.58E-03 1.65E-05 2.54E-07 1.65E-04 9.83E-07 0 3.09E-06 2.94E-06 1.27E-07 2.4E-04
ADPF MJ 3.54E+03 7.66E+01 5.63E-01 9.34E+01 2.82E+00 0 1.43E+01 7.88E+01 4.72E-01 -1.51E+03
m3 world eq
WDP 6.01E+01 3.38E-01 9.65E-03 8.56E+00 5.02E-03 0 6.32E-02 1.52E-01 3.1E-02 -3.41E+01
deprived
GWP = Global warming potential; ODP = Depletion potential of the stratospheric ozone layer; AP = Acidification potential of land and water; EP =
Eutrophication potential; POCP = Formation potential of tropospheric ozone photochemical oxidants; ADPE = Abiotic depletion potential for non-fossil
resources; ADPF = Abiotic depletion potential for fossil resources; WDP = Water (user) deprivation potential)
RESULTS OF THE LCA - INDICATORS TO DESCRIBE RESOURCE USE according to EN 15804+A2: 1 m² of the VELUX BA 5/6
glazing system with VENTRIA 3 system sashes
Parameter Unit A1-A3 A4 A5 B2 B6 C1 C2 C3 C4 D
PERE MJ 3.34E+02 1.19E+00 3.72E-02 8.03E+00 2.14E-02 0 2.23E-01 4.68E-01 2.45E-02 -1.94E+02
PERM MJ 8.98E-03 0 -8.98E-03 0 0 0 0 0 0 0
PERT MJ 3.34E+02 1.19E+00 2.82E-02 8.03E+00 2.14E-02 0 2.23E-01 4.68E-01 2.45E-02 -1.94E+02
PENRE MJ 3.49E+03 7.66E+01 9.87E-01 9.35E+01 2.82E+00 0 1.43E+01 7.88E+01 1.08E+02 -1.51E+03
PENRM MJ 5.38E+01 0 -2.12E-01 0 0 0 0 0 -5.36E+01 0
PENRT MJ 3.54E+03 7.66E+01 7.75E-01 9.35E+01 2.82E+00 0 1.43E+01 7.88E+01 5.41E+01 -1.51E+03
SM kg 1.09E+01 0 0 4.16E-01 0 0 0 0 0 7.71E+01
RSF MJ 0 0 0 0 0 0 0 0 0 0
NRSF MJ 0 0 0 0 0 0 0 0 0 0
FW m3 1.37E+01 2.07E-02 5.65E-04 0 6.5E-04 0 3.88E-03 1.42E-02 2.39E-03 -1.55E+00
PERE = Use of renewable primary energy excluding renewable primary energy resources used as raw materials; PERM = Use of renewable primary
energy resources used as raw materials; PERT = Total use of renewable primary energy resources; PENRE = Use of non-renewable primary energy
excluding non-renewable primary energy resources used as raw materials; PENRM = Use of non-renewable primary energy resources used as raw
materials; PENRT = Total use of non-renewable primary energy resources; SM = Use of secondary material; RSF = Use of renewable secondary fuels;
NRSF = Use of non-renewable secondary fuels; FW = Use of net fresh water
RESULTS OF THE LCA – WASTE CATEGORIES AND OUTPUT FLOWS according to EN 15804+A2:
1 m² of the VELUX BA 5/6 glazing system with VENTRIA 3 system sashes
Parameter Unit A1-A3 A4 A5 B2 B6 C1 C2 C3 C4 D
HWD kg 3.14E-02 4.82E-04 1.62E-06 4.93E-04 3.55E-06 0 9.02E-05 3.75E-04 4.23E-06 1.41E-02
NHWD kg 8.95E+01 4.87E+00 6.4E-03 3.18E+00 8.75E-03 0 9.11E-01 1.51E-01 1.32E-01 -3.98E+01
RWD kg 6.83E-03 4.49E-05 1.16E-06 1.58E-04 1.96E-05 0 8.4E-06 2.06E-04 7.63E-07 -1.08E-03
CRU kg 0 0 0 0 0 0 0 0 0 0
MFR kg 3.87E-01 0 0 4.42E-01 0 0 0 8.76E+01 0 0
7 Environmental Product Declaration - VELUX Group - VELUX glass architecture made from a BA 5/6 glazing system and VENTRIA 3 system sashes
MER kg 0 0 0 0 0 0 0 0 0 0
EEE MJ 0 0 6.82E-01 0 0 0 0 0 9.65E+00 0
EET MJ 0 0 1.17E+00 0 0 0 0 0 1.66E+01 0
HWD = Hazardous waste disposed; NHWD = Non-hazardous waste disposed; RWD = Radioactive waste disposed; CRU = Components for re-use;
MFR = Materials for recycling; MER = Materials for energy recovery; EEE = Exported electrical energy; EET = Exported thermal energy
RESULTS OF THE LCA – additional impact categories according to EN 15804+A2-optional:
1 m² of the VELUX BA 5/6 glazing system with VENTRIA 3 system sashes
Parameter Unit A1-A3 A4 A5 B2 B6 C1 C2 C3 C4 D
Disease
PM 2.67E-05 5.21E-07 1.93E-09 3.82E-07 1.71E-09 0 9.74E-08 1.01E-06 3.28E-09 -1.33E-05
incidence
IR kBq U235 eq 5.49E+00 3.96E-02 7.28E-04 1.35E-01 8.12E-03 0 7.41E-03 9.15E-02 6.12E-04 -7.43E-01
ETP-fw CTUe 1.71E+03 4.05E+01 2.11E-01 4.36E+01 3.45E-01 0 7.57E+00 2.87E+01 1.02E+01 -8.04E+02
HTP-c CTUh 5.69E-07 2.86E-09 7.86E-11 1.58E-08 4.51E-11 0 5.34E-10 1.51E-09 2.2E-10 -8.15E-08
HTP-nc CTUh 7.41E-06 7.6E-08 5.17E-10 1.94E-07 2.39E-09 0 1.42E-08 4.16E-08 3.69E-09 5.26E-07
SQP SQP 9.42E+02 5.75E+01 1.01E-01 2.54E+01 2.41E-01 0 1.08E+01 5.55E+00 1.69E-01 -3.87E+02
PM = Potential incidence of disease due to PM emissions; IR = Potential Human exposure efficiency relative to U235; ETP-fw = Potential comparative
Toxic Unit for ecosystems; HTP-c = Potential comparative Toxic Unit for humans (cancerogenic); HTP-nc = Potential comparative Toxic Unit for humans
(not cancerogenic); SQP = Potential soil quality index
Disclaimer 1 – for the indicator “Potential Human exposure efficiency relative to U235”. This impact category deals mainly with the
eventual impact of low-dose ionizing radiation on human health of the nuclear fuel cycle. It does not consider effects due to possible
nuclear accidents, occupational exposure or radioactive waste disposal in underground facilities. Potential ionizing radiation from the
soil, radon and from some construction materials is also not measured by this indicator.
Disclaimer 2 – for the indicators “abiotic depletion potential for non-fossil resources”, “abiotic depletion potential for fossil resources”,
“water (user) deprivation potential, deprivation-weighted water consumption”, “potential comparative toxic unit for ecosystems”,
“potential comparative toxic unit for humans – cancerogenic”, “Potential comparative toxic unit for humans - not cancerogenic”,
“potential soil quality index”. The results of this environmental impact indicator shall be used with care as the uncertainties on these
results are high as there is limited experience with the indicator.
6. LCA: Interpretation
Figure 1 illustrates the relative contributions of the different 3-layered glazing.
modules along the life cycle for VELUX glass architecture with
Figure 1: Relative environmental impacts of the different By far the largest part of environmental impacts is caused
life cycle stages for VELUX glass architecture with 3- during production (modules A1–A3) of the glass architecture.
layered glazing (modules A1–A3 = 100 %) The other life cycle stages including operational energy use are
8 Environmental Product Declaration - VELUX Group - VELUX glass architecture made from a BA 5/6 glazing system and VENTRIA 3 system sashes
comparably small. replacement of the motor; hazardous and radio-active waste
are mainly caused by the European electricity mix used during
Benefits and burdens beyond the system boundary (module D) the use phase.
are in the order of 35 % to 55 % of the impacts over the product
life cycle (modules A1–C4). The net positive impact ('load') of A representative glass building project from 2016 was scaled to
the ADPelements is related to copper input as the copper the declared unit, as there is no typical functional unit due to
cathode for the remelting of recycled aluminium. the high number of variants. Where possible, the worst-case
approach was followed. This means that the worst values or
The use of renewable primary energy is mainly caused by the assumptions were used in this analysis to determine the
share of renewable energy in the electricity mix; thus, the material and energy flows; e.g., the version with 3-layered
production stage is the main driver of this impact category; the insulation glass is declared.
same holds also for the use of non-renewable primary energy. The representative glass architecture system consists of a total
of 1097 m² roof area including 32 VENTRIA 3 system sashes
Material use of primary energy is negligible and related to (max. area 4 m2/VENTRIA 3).
plastic parts of the product and packaging material. The
material use of primary energy is transferred to its energy use This EPD is also considered representative for the version with
when the materials containing primary energy are incinerated 2-layered glazing. The declared values for this version are 10 %
with energy recovery. to 15 % lower than the declared values due to lower material
intensity. Only the values for the ADPelements are higher for
Non-hazardous waste as the quantitatively most relevant waste the 2-layered version, due to the different types of glazing.
flows is mainly caused during maintenance due to the
7. Requisite evidence
7.1 Formaldehyde Not applicable; no test defined in applicable product standards.
No test defined in applicable product standards.
7.4 Fire gas toxicity
7.2 MDI No test defined in applicable product standards.
No test defined in applicable product standards.
7.5 VOC emissions
7.3 Checking for pretreatment of the substances used No test defined in applicable product standards.
(Measurement according to AltholzV)
8. References
Product category rules of IBU
EN 13830
IBU (2021) DIN EN 13830:2020-11, Curtain walling - Product standard.
IBU (2021): General Instructions for the EPD Programme of the
Institut Bauen und Umwelt e.V. Version 2.0, Institut Bauen und ISO 14001
Umwelt, Berlin. DIN EN ISO 14001:2015: Environmental management
systems - Requirements with guidance for use.
IBU (2021)
IBU (2021): PCR Part A: Calculation rules for the life cycle EN 14351-1
assessment and requirements on the project report according DIN EN 14351-1:2016-12, Windows and doors - Product
to EN 15804+A2. Version 1.3, Institut Bauen und Umwelt e.V., standard, performance characteristics - Part 1: Windows and
Berlin. external pedestrian doorsets.
IBU (2023) EN 15804
IBU (2023): PCR Part B: Requirements on the EPD for DIN EN 15804+A2:2022-03, sustainability of construction
windows and doors. Version 2023/04, Institut Bauen und works - Environmental product declarations - Core rules for the
Umwelt e.V., Berlin. product category construction products; German version EN
15804: 2012+A2:2019 + AC:2021.
Standards and legal documents
EN 16485
EN 12101-2 DIN EN 16485:2014-07, Round and sawn timber -
DIN EN 12101-2:2017-08, Smoke and heat control systems - Environmental Product Declarations - Product category rules
Part 2: Natural smoke and heat exhaust ventilators. for wood and wood-based products for use in construction;
German version EN 16485:2014.
EN 12207
DIN EN 12207:2017-03, Windows and doors - Air permeability ISO 9001
– Classification. DIN EN ISO 9001:2015, Quality management systems -
Requirements.
EN 12208
DIN EN 12208:2000-06, Windows and doors - Watertightness – ISO 14025
Classification. DIN EN ISO 14025:2006-07, Environmental labels and
declarations - Type III Environmental declarations - Principles
EN 12210 and procedures.
DIN EN 12210:2016-09, Windows and doors - Resistance to
wind load – Classification.
9 Environmental Product Declaration - VELUX Group - VELUX glass architecture made from a BA 5/6 glazing system and VENTRIA 3 system sashes
ISO 14044 products and repealing Council Directive 89/106/EEC.
DIN EN ISO 14044:2006-07, Environmental management - Life
cycle assessment - Requirements and guidance. COUNCIL REGULATION (EU) No 333/2011
COUNCIL REGULATION (EU) No 333/2011 of 31 March 2011
ISO 45001 establishing criteria determining when certain types of scrap
ISO 45001:2018-03, Occupational health and safety metal cease to be waste under Directive 2008/98/EC of the
management systems - Requirements with guidance for use. European Parliament and of the Council.
Building authority approval No. Z-14.4-486 European Waste List (Waste index)
Allgemeine bauaufsichtliche Zulassung/Allgemeine http://www.gesetze-im-internet.de/avv/anlage.htmEN 16485
Bauargenehmigung, Nr. Z-14.4-486, für Klemmverbindungen
und ihre Produkte für die Fassadensysteme BA 5 und BA 6, Additional references
gültig vom 14.9.2020 bis 14.9.2025.
brands & values 2017
ECHA candidate list brands & values (2017): Hintergrundbericht; Ökobilanz nach
The candidate list of substances of very high concern, DIN EN ISO 14040 & 14044 für eine Glasarchitektur aus BA
European Chemicals Agency, Helsinki. Available at: 5/6-Verglasungssystem und VENTRIA 3 Systemflügeln der
https://echa.europa.eu/nl/-/four-newsubstances-added-to-the Firma JET Brakel Aero GmbH. Berichtsdatum: 04.01.2017,
candidate-list. erstellt durch: brands & values GmbH, Bremen, in
Zusammenarbeit mit JET Brakel Aero GmbH.
Regulation on biocidal products
REGULATION (EU) No 528/2012 OF THE EUROPEAN CEWEP Energy Report III
PARLIAMENT AND OF THE COUNCIL of 22 May 2012 Reimann D.O. (2013): CEWEP Energy Report III (Status 2007
concerning the making available on the market and use of – 2010); Results of Specific Data for Energy, R1 Plant
biocidal products. Efficiency Factor and NCV of 314 European Waste-to-Energy
(WtE) Plants. CEWEP, Würzburg/Brussels, 2013.
Regulation (EU) Nr. 305/2011(CPR)
REGULATION (EU) No 305/2011 OF THE EUROPEAN ecoinvent v3.9.1
PARLIAMENT AND OF THE COUNCIL of 9 March 2011 laying ecoinvent v3.9.1, LCA database, 12/2022. Ecoinvent centre,
down harmonised conditions for the marketing of construction Zürich.
10 Environmental Product Declaration - VELUX Group - VELUX glass architecture made from a BA 5/6 glazing system and VENTRIA 3 system sashes
Publisher
Institut Bauen und Umwelt e.V. +49 (0)30 3087748- 0
Hegelplatz 1 info@ibu-epd.com
10117 Berlin www.ibu-epd.com
Germany
Programme holder
Institut Bauen und Umwelt e.V. +49 (0)30 3087748- 0
Hegelplatz 1 info@ibu-epd.com
10117 Berlin www.ibu-epd.com
Germany
Author of the Life Cycle Assessment
Dr. Frank Werner - Umwelt & Entwicklung + 41 (0)44 241 39 06
Kammelenbergstrasse 30 frank@frankwerner.ch
9011 St. Gallen http://www.frankwerner.ch/
Switzerland
Owner of the Declaration
VELUX Group +4545164871
Ådalsvej 99 birthe.kjeldsen@velux.com
2970 Hørsholm www.velux.com
Denmark
11 Environmental Product Declaration - VELUX Group - VELUX glass architecture made from a BA 5/6 glazing system and VENTRIA 3 system sashes
