ENVIRONMENTAL PRODUCT DECLARATION
as per ISO 14025 and EN 15804+A2
Owner of the Declaration VELUX Group
Publisher Institut Bauen und Umwelt e.V. (IBU)
Programme holder Institut Bauen und Umwelt e.V. (IBU)
Declaration number EPD-VEL-20210075-CCI3-EN
Issue date 04/05/2021
Valid to 03/05/2026
VELUX Modular Skylight (double glazing configuration)
VELUX Group
www.ibu-epd.com | https://epd-online.com
General Information
VELUX Group VELUX Modular Skylight (double glazing
configuration)
Programme holder Owner of the declaration
IBU – Institut Bauen und Umwelt e.V. VELUX Group
Hegelplatz 1 Ådalsvej 99
10117 Berlin 2970 Hørsholm
Germany Denmark
Declaration number Declared product / declared unit
EPD-VEL-20210075-CCI3-EN The declared unit is a window of one square meter (m2) with double
glazing configuration.
The declared unit is based on the configuration of a standard size window
measuring 1.23 m * 1.48 m.
This declaration is based on the product category rules: Scope:
Windows and doors , 01/08/2021 The EPD is a representative EPD covering VELUX Modular System (VMS)
(PCR checked and approved by the SVR) products. The products are manufactured by VELUX Group in Østbirk,
Denmark for sale throughout Europe.
The owner of the declaration shall be liable for the underlying information
Issue date and evidence; the IBU shall not be liable with respect to manufacturer
information, life cycle assessment data and evidences.
04/05/2021
The EPD was created according to the specifications of EN 15804+A2. In
the following, the standard will be simplified as EN 15804.
Valid to
03/05/2026 Verification
The standard EN 15804 serves as the core PCR
Independent verification of the declaration and data according to ISO
14025:2011
internally X externally
Dipl.-Ing. Hans Peters
(Chairman of Institut Bauen und Umwelt e.V.)
Florian Pronold Juliane Franze,
(Managing Director Institut Bauen und Umwelt e.V.) (Independent verifier)
1 Environmental Product Declaration - VELUX Group - VELUX Modular Skylight (double glazing configuration)
Product
Name Value Unit
Product description/Product definition
Fire resistance class § 4.4.1 B-s1.d0 class
VELUX Modular Skylights (VMS) are sash-frame constructed
Air permeability , § 4.14 4 class
single roof windows. The modules fit together and can be
configured in several predefined daylight solutions. All Resistance to wind load, § 4.2
individual skylights are delivered as prefabricated modules with (for window width >1000 mm or
C5 class
dedicated factory finished flashings to ensure watertightness in height > 2400 mm no
every solution. performance is determined)
The VMS include modules, which can be opened (venting) as 8 mm toughened -
well as modules, which cannot be opened (fixed). The EPD 16 mm -10.76 mm
Resistance to snow loads, § 4.3 mm
covers VMS modules in sizes from 0.405 m2 up to 2.3 m2. (55.2) laminated
float
The glass panes are with double glazing and different glass Watertightness, § 4.5 E1200 class
configurations are covered by the EPD. The glass thickness
Impact resistance, § 4.7 (for
ranges from 12 to 18 mm. The glass panes have cavities filled
window width >550 mm or
with Argon gas. The representative glass configuration used for test is passed -
height > 778 mm no
the EPD calculations has 8 mm toughened glass, 16mm space
performance is determined)
and 10mm laminated glass. This configuration is conservative
Load bearing capacity of safety
with regards to the environmental impact results. For the test is passed -
devices, § 4.8
placing on the market of the product in the European
Acoustic performance, § 4.11 38 (-1; -4) -
Union/European Free Trade Association (EU/EFTA) (with the
exception of Switzerland) Regulation (EU) No. 305/2011 (CPR) Thermal transmittance, § 4.12 ,
applies. The product needs a declaration of performance taking 90 degree installation acc. to EN 1,4 W/(m2K)
into consideration EN 14351-1:2006+A2:2016, Windows and 10077-1/2
doors - Product standard, performance characteristics - Part 1: Solar factor, § 4.13 0.51 -
Windows and external pedestrian doorsets. For the application Light transmittance, § 4.13 0.73 -
and use, the respective national provisions apply.
Product performance data in accordance with DS/EN 14351-
Application 1:2006+A2:2016, Windows and doors - Product standard,
VELUX Modular Skylight consists of modules, that are built performance characteristics - Part 1: Windows and external
together to form a long band of window modules in several pedestrian doorsets.
predefined solutions such as a longlight or ridgelight. The
Base materials/Ancillary materials
length of the band of modules is determined by the need of the
individual building. Name ValueUnit
Glass pane 72 %
Technical Data
Composite frame of glass fibre reinforced
The Declaration of Performance including relevant technical 17 %
polyurethane
specifications and test methods/test standards can be
Metals 9 %
downloaded from the website www.velux.com/ce-marking.
Other materials 3 %
The performance values are specific for the specific VMS
variants covered by the EPD.
The declared values in below table relate to the reference Recycled content
product incl. the pane variant 10T. For other VMS product
variants, specific values can be selected at the bottom of the
above-mentioned download page.
Constructional data (Reference product incl. pane variant
10T)
The values stated in the table relate to the recycled material
streams in VELUX production.
Reference service life
No reference service life (RSL) is defined for the VMS products
because the use stage modules are not included in the EPD.
LCA: Calculation rules
(reference window based on EN 14351-1) with double glazed
Declared Unit window panes.
Multiple product dimensions are represented by this EPD as
Declared unit
specified in the product description.
Name Value Unit
The declared unit is 1 m2 window calculated based on one Declared unit 1 m2
representative window module measuring 1.23 m * 1.48 m Weight per piece 57.78 kg/pce
2 Environmental Product Declaration - VELUX Group - VELUX Modular Skylight (double glazing configuration)
A data quality and a sensitivity analysis shows that the results End of life stage:
are robust with regards to data quality and appropriateness.
• C1 - De-construction: de-construction of the window
There is low variability of production processes and product
with the use of a screwdriver
variations have a limited influence on the results. This also
applies with regards to the size of the windows where larger • C2 - Transport: transport of window materials to
sizes have slightly lower environmental impacts compared with incineration and recycling
smaller sizes and the other way around. • C3 - Waste processing: sorting of glass waste,
incineration of plastic and rubber parts
System boundary
• C4 - Disposal: disposal of all materials
Type of EPD: Cradle to gate - with options. The following life
cycle phases were considered:
Product stage:
Benefits and loads beyond the system boundaries:
• A1 - Raw material extraction and processing: production
• D - Reuse, recovery and recycling potential: benefits
of the pre-products (e.g. glass pane profiles, covers,
from plastic incineration processes and recycling of
brackets, sealant...) and packaging components
metal and glass. For details, see scenario information
(primarily wood)
under 'Scenarios and additional technical information'.
• A2 - Transport to the manufacturer:
Transport of pre-products and packaging components to Geographic Representativeness
the manufacturing site Land or region, in which the declared product system is
• A3 - Manufacturing: The composite profiles for the manufactured, used or handled at the end of the product´s
products are produced at VELUX production site in lifespan: Denmark
Grindsted in Denmark in a pultrusion process. The final
assembly and production of the VMS modules takes
Comparability
place at the VELUX production site in Østbirk in
Basically, a comparison or an evaluation of EPD data is only
Denmark. The final production processes include
possible if all the data sets to be compared were created
shortening of profiles, drilling of holes, clamping and
according to EN 15804 and the building context, respectively
glueing, mounting of gaskets, brackets, panes etc. as
the product-specific characteristics of performance, are taken
well as stacking on pallets.
into account.
LCA: Scenarios and additional technical information
Characteristic product properties of biogenic carbon
End of life (C1-C4)
2.3 kg wood packaging is used per declared unit. This is the
only biogenic material used. Name Value Unit
Collected as mixed construction waste 105 kg
Information describing the biogenic Carbon Content at
factory gate Recycling 31 kg
Name ValueUnit Energy recovery 3 kg
kg Landfilling 71 kg
Biogenic carbon content in product -
C
Reuse, recovery and/or recycling potentials (D), relevant
Biogenic carbon content in accompanying kg
1 scenario information
packaging C
The recycling efficiency for all materials is maximum 90% in
Note: 1 kg of biogenic carbon is equivalent to 44/12 kg of CO . accordance with EN 17213. This means that only 90% of the
2
recycled materials substitute primary materials. Secondary
materials in the VMS modules do not substitute primary
The construction process stage and the use stage modules are materials in the end-of-life scenario. The recycled glass is used
not declared. However, the quantity of packaging generated in as container glass in the end-of-life scenario.
module A5 is declared as scenario information. Name Value Unit
Installation into the building (A5) Glass recycled 30 %
Name Value Unit Metal recycled 95 %
Wood packaging for waste treatment 2.3 kg Plastic incinerated with energy recovery 95 %
Plastic packaging for waste treatment 0.07 kg
Metal screws for waste treatment 0.02 kg
3 Environmental Product Declaration - VELUX Group - VELUX Modular Skylight (double glazing configuration)
LCA: Results
Disclaimer:
EP-freshwater: This indicator has been calculated as 'kg P eq' as required in the characterization model (EUTREND model, Struijs et
al., 2009b, as implemented in ReCiPe; http://eplca.jrc.ec.europa.eu/LCDN/developerEF.xhtml)
DESCRIPTION OF THE SYSTEM BOUNDARY (X = INCLUDED IN LCA; MND = MODULE OR INDICATOR NOT DECLARED; MNR
= MODULE NOT RELEVANT)
Benefits and
Construction loads beyond
Product stage Use stage End of life stage
process stage the system
boundaries
la ire ta m w a Ry lp p u s tro p s n a rT g n iru tc a fu n a M e h t m o rf tro p s n a rTe tis e h t o t e ta g y lb m e s s A e s U e c n a n e tn ia M ria p e R tn e m e c a lp e R tn e m h s ib ru fe R y g re n e la n o ita re p Oe s u re ta w la n o ita re p Oe s u n o itc u rts n o c -e Dn o itilo m e d tro p s n a rT g n is s e c o rp e ts a W la s o p s iD -e s u e R-y re v o c e R-g n ilc y c e Rla itn e to p
A1 A2 A3 A4 A5 B1 B2 B3 B4 B5 B6 B7 C1 C2 C3 C4 D
X X X MND MND MND MND MNR MNR MNR MND MND X X X X X
RESULTS OF THE LCA - ENVIRONMENTAL IMPACT according to EN 15804+A2: 1 m2 VMS with double glazing
Parameter Unit A1 A2 A3 C1 C2 C3 C4 D
GWP-total kg CO 2 eq 1.74E+02 3.86E+00 3.93E+00 1.85E-03 1.02E-01 3.38E+00 1.21E+00 -2.48E+01
GWP-fossil kg CO 2 eq 1.74E+02 3.84E+00 7.8E+00 1.84E-03 1.01E-01 3.38E+00 1.26E+00 -2.48E+01
GWP-biogenic kg CO 2 eq 1.94E-01 -6.54E-03 -3.88E+00 6.14E-06 -1.72E-04 8.53E-04 -5.68E-02 -2.88E-02
GWP-luluc kg CO 2 eq 4.35E-02 3.1E-02 1.16E-02 2.67E-06 8.15E-04 1.12E-04 2.79E-03 -7.8E-03
ODP kg CFC11 eq 8.4E-08 4.6E-16 3.61E-09 4.05E-17 1.21E-17 1.34E-08 3.26E-15 -3.28E-14
AP mol H+ eq 3.21E+01 1.27E-02 1.21E-02 4.07E-06 3.33E-04 2.25E-03 5.7E-03 -1.24E-01
EP-freshwater kg P eq 2.21E+00 1.16E-05 4.36E-05 4.92E-09 3.06E-07 3.24E-05 1.3E-04 -1.15E-05
EP-marine kg N eq 3.84E-02 5.73E-03 4.27E-03 9.04E-07 1.51E-04 9.71E-04 1.47E-03 -2.75E-02
EP-terrestrial mol N eq 4.09E-01 6.4E-02 4.44E-02 9.49E-06 1.68E-03 1.13E-02 1.61E-02 -3.09E-01
kg NMVOC
POCP 1.51E+00 1.12E-02 1.13E-02 2.48E-06 2.94E-04 2.56E-03 4.36E-03 -6.58E-02
eq
ADPE kg Sb eq 1.81E-03 2.75E-07 6.64E-06 5.33E-10 7.22E-09 1.13E-07 9.57E-08 -8.27E-06
ADPF MJ 2.51E+03 5.1E+01 9.79E+01 3.24E-02 1.34E+00 2.32E+00 1.75E+01 -3.1E+02
m3 world eq
WDP 4.35E+00 3.42E-02 -5.58E-02 4.02E-04 9E-04 3.84E-01 3.97E-02 -1.93E+00
deprived
GWP = Global warming potential; ODP = Depletion potential of the stratospheric ozone layer; AP = Acidification potential of land and water; EP =
Eutrophication potential; POCP = Formation potential of tropospheric ozone photochemical oxidants; ADPE = Abiotic depletion potential for non-fossil
resources; ADPF = Abiotic depletion potential for fossil resources; WDP = Water (user) deprivation potential)
RESULTS OF THE LCA - INDICATORS TO DESCRIBE RESOURCE USE according to EN 15804+A2: 1 m2 VMS with double
glazing
Parameter Unit A1 A2 A3 C1 C2 C3 C4 D
PERE MJ 5.48E+02 2.87E+00 9.14E+01 1.44E-02 7.54E-02 2.33E-01 1.56E+00 -5.72E+01
PERM MJ 0 0 3.92E+01 0 0 0 0 0
PERT MJ 5.48E+02 2.87E+00 1.31E+02 1.44E-02 7.54E-02 2.33E-01 1.56E+00 -5.72E+01
PENRE MJ 2.78E+03 5.1E+01 9.51E+01 3.24E-02 1.34E+00 7.74E+01 1.75E+01 -3.1E+02
PENRM MJ 1.47E+02 0 2.83E+00 0 0 -7.51E+01 0 0
PENRT MJ 2.93E+03 5.1E+01 9.8E+01 3.24E-02 1.34E+00 2.32E+00 1.75E+01 -3.1E+02
SM kg 2.78E+00 0 2.32E-02 0 0 0 0 0
RSF MJ 1.52E-12 0 0 0 0 0 0 0
NRSF MJ 1.78E-11 0 0 0 0 0 0 0
FW m3 7.02E+02 3.32E-03 4.07E-02 1.66E-05 8.73E-05 9.04E-03 1.69E-03 -1.47E-01
PERE = Use of renewable primary energy excluding renewable primary energy resources used as raw materials; PERM = Use of renewable primary
energy resources used as raw materials; PERT = Total use of renewable primary energy resources; PENRE = Use of non-renewable primary energy
excluding non-renewable primary energy resources used as raw materials; PENRM = Use of non-renewable primary energy resources used as raw
materials; PENRT = Total use of non-renewable primary energy resources; SM = Use of secondary material; RSF = Use of renewable secondary fuels;
NRSF = Use of non-renewable secondary fuels; FW = Use of net fresh water
RESULTS OF THE LCA – WASTE CATEGORIES AND OUTPUT FLOWS according to EN 15804+A2:
1 m2 VMS with double glazing
Parameter Unit A1 A2 A3 C1 C2 C3 C4 D
HWD kg 3.48E-03 2.38E-06 2.17E-07 1.34E-11 6.25E-08 1.65E-09 1.97E-07 -2.46E-07
NHWD kg 6.04E+01 7.81E-03 3.44E-01 2.3E-05 2.05E-04 3.93E+01 3.9E+01 -3.65E+00
RWD kg 1.92E-01 6.32E-05 3.33E-03 4.92E-06 1.66E-06 3.72E-05 1.9E-04 -1.06E-02
CRU kg 0 0 0 0 0 0 0 0
MFR kg 6.24E+00 0 0 0 0 1.71E+01 0 0
4 Environmental Product Declaration - VELUX Group - VELUX Modular Skylight (double glazing configuration)
MER kg 0 0 0 0 0 1.4E+00 0 0
EEE MJ 0 0 0 0 0 6.1E+00 0 0
EET MJ 0 0 0 0 0 1.1E+01 0 0
HWD = Hazardous waste disposed; NHWD = Non-hazardous waste disposed; RWD = Radioactive waste disposed; CRU = Components for re-use;
MFR = Materials for recycling; MER = Materials for energy recovery; EEE = Exported electrical energy; EET = Exported thermal energy
RESULTS OF THE LCA – additional impact categories according to EN 15804+A2-optional:
1 m2 VMS with double glazing
Parameter Unit A1 A2 A3 C1 C2 C3 C4 D
Disease
PM 2E-06 6.8E-08 5.93E-07 3.41E-11 1.79E-09 1.34E-08 6.23E-08 -1.04E-06
incidence
IR kBq U235 eq 3.94E+00 9.13E-03 3.52E-01 8.07E-04 2.4E-04 2.16E-02 2.44E-02 -2.05E+00
ETP-fw CTUe 4.57E+02 3.6E+01 2.56E+01 1.39E-02 9.47E-01 1.33E+00 1.45E+01 -2.44E+02
HTP-c CTUh 3.04E-07 7.55E-10 4.9E-08 3.83E-13 1.98E-11 6.01E-11 9.67E-10 -1.42E-08
HTP-nc CTUh 1.34E-06 4.43E-08 5.12E-08 1.41E-11 1.16E-09 2.65E-09 9.19E-08 -2.29E-07
SQP SQP 1.33E+02 1.79E+01 1.09E+03 1.03E-02 4.7E-01 1.98E+00 2.46E+00 -1.34E+01
PM = Potential incidence of disease due to PM emissions; IR = Potential Human exposure efficiency relative to U235; ETP-fw = Potential comparative
Toxic Unit for ecosystems; HTP-c = Potential comparative Toxic Unit for humans (cancerogenic); HTP-nc = Potential comparative Toxic Unit for humans
(not cancerogenic); SQP = Potential soil quality index
Disclaimer 1 – for the indicator IRP. This impact category deals mainly with the eventual impact of low dose ionizing radiation on human
health of the nuclear fuel cycle. It does not consider effects due to possible nuclear accidents, occupational exposure nor due to
radioactive waste disposal in underground facilities. Potential ionizing radiation from the soil, from radon and from some construction
materials is also not measured by this indicator.
Disclaimer 2 – for the indicators ADPE, ADPF, WDP, ETP-fw, HTP-c, HTP-nc, SQP. The results of this environmental impact indicator
shall be used with care as the uncertainties on these results are high or as there is limited experience with the indicator.
References
EN 14351-1 ISO 10077-2
EN 14351-1:2006+A2:2016, Windows and doors - Product ISO 10077-2:2017, Thermal performance of windows, doors
standard, performance characteristics - Part 1: and shutters - Calculation of termal transmittance - Part 2:
Windows and external pedestrian doorsets. Numerical method for frames.
EN 15804 ISO 14025
EN 15804:2019+A2: Sustainability of construction works - DIN EN ISO 14025:2011-10, Environmental labels and
Environmental Product Declarations - Core rules for the product declarations - Type III environmental declarations - Principles
category of construction products. and procedures.
EN 17213 Regulation (EU) No. 305/2011
EN 17213:2020: 'Windows and doors – Environmental Product REGULATION (EU) No 305/2011 OF THE EUROPEAN
Declarations – Product category rules for windows and PARLIAMENT AND OF THE COUNCIL of 9 March 2011 laying
pedestrian doorsets'. down harmonised conditions for the marketing of construction
products and repealing Council Directive 89/106/EEC.
IBU PCR Part A
IBU PCR Part A: Institut Bauen und Umwelt e.V., Product GaBi LCA software and database
Category Rules for Building-Related Products and Services. The LCA modelling software is GaBi program version 9.5.2.49
Calculation Rules for the Life Cycle Assessment and with corresponding databases from Sphera Solutions GmbH.
Requirements on the Project Report according to EN Documentation hyperlink www.gabi-software.com/support/gabi.
15804+A2:2019.
IBU 2016
ISO 10077-1 Institut Bauen und Umwelt e.V.: General Programme
ISO 10077-1:2017, Thermal performance of windows, doors Instructions for the Preparation of EPDs at the Institut Bauen
and shutters - Calculation of termal transmittance - Part 1: und Umwelt e.V. Version 1., Berlin: Institut Bauen und Umwelt
General. e.V., 2016. Hyperlinks: http://www.ibu-epd, www.ibu-epd.com.
5 Environmental Product Declaration - VELUX Group - VELUX Modular Skylight (double glazing configuration)
Publisher
Institut Bauen und Umwelt e.V. +49 (0)30 3087748- 0
Hegelplatz 1 info@ibu-epd.com
10117 Berlin www.ibu-epd.com
Germany
Programme holder
Institut Bauen und Umwelt e.V. +49 (0)30 3087748- 0
Hegelplatz 1 info@ibu-epd.com
10117 Berlin www.ibu-epd.com
Germany
Author of the Life Cycle Assessment
FORCE Technology +4543250856
Park Alle 345 chme@force.dk
2605 Brøndby www.forcetechnology.com
Denmark
Owner of the Declaration
VELUX Group +4545164726
Ådalsvej 99 jakob.roerbech@velux.com
2970 Hørsholm www.velux.com
Denmark
6 Environmental Product Declaration - VELUX Group - VELUX Modular Skylight (double glazing configuration)
