ENVIRONMENTAL PRODUCT DECLARATION
as per ISO 14025 and EN 15804+A2
Owner of the Declaration VELUX Group
Publisher Institut Bauen und Umwelt e.V. (IBU)
Programme holder Institut Bauen und Umwelt e.V. (IBU)
Declaration number EPD-VEL-20220133-IBJ3-EN
Issue date 25.07.2022
Valid to 24.07.2027
VELUX flat roof window CFP
VELUX A/S
www.ibu-epd.com | https://epd-online.com
1. General Information
VELUX A/S VELUX flat roof window CFP
Programme holder Owner of the declaration
IBU – Institut Bauen und Umwelt e.V. VELUX Group
Hegelplatz 1 Ådalsvej 99
10117 Berlin 2970 Hørsholm
Germany Denmark
Declaration number Declared product / declared unit
EPD-VEL-20220133-IBJ3-EN The declaration represents 1 piece of a VELUX flat roof windows CFP of
the size 1.20 m x 1.20 m = 1.44 m2
This declaration is based on the product category rules: Scope:
Windows and doors , 01.08.2021 The declaration covers 100% of VELUX flat roof windows CFP by
(PCR checked and approved by the SVR) Partizánske Building Components SK, Slovenia.
The owner of the declaration shall be liable for the underlying information
and evidence; the IBU shall not be liable with respect to manufacturer
Issue date information, life cycle assessment data and evidences.
25.07.2022
The EPD was created according to the specifications of EN 15804+A2. In
the following, the standard will be simplified as EN 15804.
Valid to
Verification
24.07.2027
The standard EN 15804 serves as the core PCR
Independent verification of the declaration and data according to ISO
14025:2011
internally X externally
Dipl.-Ing. Hans Peters
(Chairman of Institut Bauen und Umwelt e.V.)
Florian Pronold Dr. Eva Schmincke,
(Managing Director Institut Bauen und Umwelt e.V.) (Independent verifier)
1 Environmental Product Declaration - VELUX A/S - VELUX flat roof window CFP
2. Product
laminated glass 35 %
2.1 Product description/Product definition tempered glass 20 %
The Velux Flat roof windows CFP consists of a fixed base unit others
made of a PVC curb with an integrated glazing unit and a top
unit with one-layer opaque or transparent acrylic (PMMA) Composition of the top unit (ISD 0000A):
dome. For the placing on the market of the product in the PMMA 95 %
European Union/European Free Trade Association (EU/EFTA) iron & cast iron 5 %
(with the exception of Switzerland) Regulation (EU) No.
305/2011 (CPR) applies. The product needs a declaration of 1) 'This product/article/at least one partial article contains
performance taking into consideration EN 1873:2005, substances listed in the candidate list (date: 02.03.2022)
Prefabricated accessories for roofing - Individual rooflights of exceeding 0.1 percentage by mass:
plastics - Product specification and test methods and the CE-
• no
marking. For the application and use the respective national
2) 'This product/article/at least one partial article contains other
provisions apply.
CMR substances in categories 1A or 1B which are not on the
2.2 Application candidate list, exceeding 0.1 percentage by mass:
Velux flat roof windows CFP are used in renovation and new • not investigated with suppliers
build. 3) 'Biocide products were added to this construction product or
it has been treated with biocide products (this then concerns a
2.3 Technical Data treated product as defined by the (EU) Regulation on Biocidal
The Declaration of Performance including relevant technical Products No. 528/2012):
specifications and test methods/test standards can be
• no
downloaded from the website www.velux.com/ce.
Recycled content
The declared values in the table relate to the reference product
incl. an average pane. For other covered product variants,
specific values can be selected at the bottom of the above-
mentioned download page
Constructional data for CFP 120120 73Q+ISD 0000
For other The values stated in the table relate to the recycled material
variants, see velux.com/ce streams in VELUX production.
Name Value Unit
2.6 Manufacture
Reaction to fire - class
Base unit:
Resistance to upward load EN 1875 UL 1500 -
water permeability acc. to EN 13985, EN PVC profiles and gaskets are produced outside Velux.
- class
1027
Resistance to downward load EN 1873 UL 2500 - The insulating glass unit is assembled at a production site in
France.
Resistance to fire EN 13501-2 NPD -
External fire performance EN 13501-5 NPD -
The production and final assembly of the base unit take place
Water tightness EN 1873 passed - on the production site in Slovakia.
Impact resistance - small hard body passed
passed -
EN 1873 The final production processes includes preparation of the PVC
Impact resistance - large soft body EN 1873 SB 1200 - frame/sash profiles by cutting, milling and drilling and
installation of EPS foam. The final PVC base is assembled by
Direct airborne sound insulation EN ISO 36 (-1;-
dB cutting, deburring and welding, cutting and mounting of gaskets
410-3 4)
and installation of the glazing unit as well as packaging,
Thermal transmittance EN 1873 0,80 W/(m2K)
stacking and wrapping of the product on pallets.
Luminous transmittance EN 410 0,72 -
Air permability EN 1026 A3 Class Top unit:
Durability EN 1873 NPD -
The plastic dome is produced and assembled on a production
Performance data of the product in accordance with the
site in Germany.
declaration of performance with respect to its essential
characteristics according to
The final production processes include forming/blow moulding
• EN 1873:2005, Prefabricated accessories for roofing - of the plastic dome, with afterwards deburring, engraving and
Individual rooflights of plastics - Product specification assembly, as well as packaging, stacking and wrapping of the
and test methods product on pallets.
The factories are ISO 9001 certified.
2.4 Delivery status
The product is available in pre-defined sizes covering 0,6x0,6m 2.7 Environment and health during manufacturing
to 1,5x1,5m. All factories are ISO 14001 and ISO 45001 certified.
2.5 Base materials/Ancillary materials 2.8 Product processing/Installation
Composition of the base unit CFP: The product is delivered to the customer in two parts, a top and
PVC 40 % bottom part. After the hole in the roof is prepared, the bottom
2 Environmental Product Declaration - VELUX A/S - VELUX flat roof window CFP
part of the product can be installed with the use of a Name Value
screwdriver, after which the top unit can be fastened to the
Building material class B
bottom unit.
Burning droplets s1
2.9 Packaging Smoke gas development d0
The packaging usually consists of:
- polyethylene film Water
- polystyrene foam parts In the event of unforeseen exposure to water (flood), no
- cardboard adverse effects on human health or the environment are to be
expected.
The use of other packaging materials is possible, but
insignificant in terms of quantity. Mechanical destruction
In the event of unforeseen mechanical destruction, VELUX flat
The plastic packaging (polyethylene (PE) film, polystyrene foam roof windows must be replaced; apart from potential injuries
parts) can be recycled if separated by type; alternatively, they from glass cullet, no adverse effects on human health or the
can be incinerated. environment are to be expected.
2.10 Condition of use 2.14 Re-use phase
The material composition of VELUX flat roof windows does not VELUX flat roof windows can be dismantled manually without
change over their service life. any problems. The metal parts are usually recycled, and the
plastic parts and wood are sent for thermal recycling for energy
2.11 Environment and health during use
recovery. Flat glass can be recycled whereas laminated glass is
VELUX flat roof windows do not contain any pollutants that
usually used as secondary aggregate in road construction or
could be released during use.
landfilling.
Environmental protection: According to current knowledge, 2.15 Disposal
hazards to water, air and soil cannot arise when the products VELUX flat roof windows are mostly inert and can be disposed
are used as intended. of in an appropriate landfill. However, due to the value of the
materials or the carbon content of the plastic parts and wood,
Health protection: According to current knowledge, no health recycling or energy recovery is preferable and common.
hazards or impairments are to be expected.
Waste code according to the European Waste List (Regulation
2.12 Reference service life
on the European Waste List):
It is not possible to calculate the reference service life
according to ISO 15686. The service life based on a
17 02 02 glass
manufacturer's declaration is 30 years. The corresponding
17 02 03 plastics
utilization scenario is declared in 4.
17 04 14 mixed metals
2.13 Extraordinary effects
2.16 Further information
Fire
Further documentation on the products, technical data sheets,
BIM files, etc. can be found at:
Fire performance according to EN 13501:1 www.velux.com
3. LCA: Calculation rules
3.1 Declared Unit Module A4 is not declared due to large variances in transport
The declared unit is 1 piece of a VELUX flat roof window CFP distances between the production site and the construction site,
with a fixed base unit made of a PVC curb with an integrated where the product is installed.
glazing unit with 1.20 m x 1.20 m = 1.44 m2.
Module A5: The products are delivered to the construction site
Declared unit
ready to be installed. Manual installation is assumed; electricity
Name Value Unit
consumption related to electric drilling machines, screw drivers,
Declared unit 1 pce. etc. is considered to be negligible. The combustible packaging
Area 1.44 m² material (plastics, wood, etc.) is assumed to be thermally
Weight 66.8 kg treated in a municipal waste incineration plant with an efficiency
R1 < 0.6 (according to the ecoinvent dataset used); the
recovered energy is declared as exported energy. Metals and
cardboard are recycled; it is assumed that these fractions reach
3.2 System boundary
the end-of-waste state after having been sorted and
Type of EPD: Cradle to gate with options, with modules C1 –
transported (as a conservative choice) to a recycler. No
C4, and module D (A1-A3, C1-C3, D and additional modules
packaging waste is landfilled.
Modules B1 to B7 are not relevant for the product under
The production of VELUX flat roof windows (modules A1-A3)
consideration or no significant environmental impacts occur.
includes raw material extraction, energy generation, waste
treatment and all transports up to the factory gate. In
Module C1 includes manual dismantling, with no significant
accordance with COUNCIL REGULATION (EU) No 333/2011,
environmental impact.
secondary metals are modeled as part of the product system
from the moment they are available as unmixed scrap.
Module C2 comprises the transport of the dismantled VELUX
Waste or secondary fuels are not used for production.
flat roof window to a sorting plant and then to a waste
3 Environmental Product Declaration - VELUX A/S - VELUX flat roof window CFP
incineration plant for the thermally treated plastic fraction.
3.5 Background data
Modules C3/C4: given the complexity of the inventoried Ecoinvent 3.8 (2021) is used as the background database.
products, a mixed end-of-life scenario is modelled, allowing the
3.6 Data quality
different materials to follow their most likely path.
As a rule of thumb, metals are recycled and plastics are The foreground data are based on extensive and detailed data
incinerated (also due to the very limited data availability on collection at the production site. The foreground data could be
plastics recycling and its benefits); coated and uncoated flat fully linked with corresponding data records from the
glass is assumed to be recycled whereas laminated glass is background database ecoinvent 3.8.
assumed to be landfilled due to very limited recycling potential. The background data was updated in 2021. Thus, the quality of
the foreground and background data can be rated as very
Metals and flat glass recycled; it is assumed that these fractions good.
reach the end-of-waste state after having been sorted and
3.7 Period under review
transported to a recycler; laminated glass is landfilled. The
The LCA data represents the production conditions for the year
combustible material (plastics, etc.) is assumed to be thermally
2021.
treated in a municipal waste incineration plant.
3.8 Geographic Representativeness
Module D includes the benefits and burdens associated with
Land or region, in which the declared product system is
recycling metals beyond the system boundary, resulting from
manufactured, used or handled at the end of the product´s
the treatment of recycled materials from the point of end-of-
lifespan: Europe
waste to the point of substitution (as loads) and substitution of
primary resources (as benefits).
It also includes the benefits and burdens associated with 3.9 Allocation
energy recovery from plastic waste in a municipal waste No co-products are generated during the production of the
incineration plant, as modeled in Module C3. VELUX products. Sorted production scrap of the different
In Module D, only net flows of metals leaving the product metals, notably aluminium, is considered a secondary material
system are considered. with no economic value (so no burdens allocated) and
considered in the quantification of net flows leaving the product
3.3 Estimates and assumptions
system. This approach is chosen to ensure a coherent
No further assumptions and estimates relevant to the result had
quantification of net flows entering module D.
to be made beyond the points made in this chapter 3 and in
chapter 4.
No processes were modelled as part of the foreground model
that would have required an allocation of multi-input processes.
3.4 Cut-off criteria
Background datasets on municipal waste incineration plants
No data available from the company survey was neglected.
were taken from ecoinvent without any modification.
These include, among other things, material use, energy
demand (heat, electricity), packaging materials of raw materials
Allocation of reuse, recycling and recovery was avoided by the
(insofar as they are generated as waste) and product
cut-off approach in the foreground model in line with DIN EN
packaging, consumables in production, waste treatment and
15804.
the transport of all inputs and outputs.
With this approach, mass and energy flows below 1 % were 3.10 Comparability
also accounted for. No processes were neglected that would
Basically, a comparison or an evaluation of EPD data is only
have been known to the project managers and would have
possible if all the data sets to be compared were created
contributed significantly to the indicators of the impact
according to EN 15804 and the building context, respectively
assessment.
the product-specific characteristics of performance, are taken
into account.
4. LCA: Scenarios and additional technical information
addition, it shall be stated that the RSL applies to the reference
Characteristic product properties of biogenic carbon conditions only.
Information on describing the biogenic carbon content at The same holds for a service life declared by the manufacturer.
factury gate Corresponding information related to in-use conditions needs
not be provided if a service life taken from the list of service life
Name ValueUnit
by BNB is declared.
kg
Biogenic carbon content in product 0.024
C Module A5
Biogenic carbon content in accompanying kg The products are delivered to the construction site ready to be
1.92
packaging C installed. Manual installation is assumed; electricity
consumption related to electric drilling machines, screw drivers,
Note: 1 kg of biogenic carbon is equivalent to 44/12 kg of CO .
2 etc. is considered to be negligible.
The combustible packaging material (plastics, wood, etc.) is
assumed to be transported 50 km with a lorry 16-32 metric
tons, EURO6 to an incineration plant with an efficiency R1 < 0.6
(according to the ecoinvent dataset used); the recovered
energy is declared as exported energy; for its quantification an
In case a reference service life according to applicable ISO
efficiency of 25.6 % is assumed for the production of heat and
standards is declared then the assumptions and in-use
13.0 % for the production of electricity (always referring to the
conditions underlying the determined RSL shall be declared. In
lower heating value of the waste).
4 Environmental Product Declaration - VELUX A/S - VELUX flat roof window CFP
Metals and cardboard are recycled; it is assumed that these of-life scenario is modelled, allowing the different materials to
fractions reach the end-of-waste state after having been sorted follow their most likely path.
and transported (as a conservative choice) to a recycler over
150 km with a lorry 16-32 metric tons, EURO6. It should also be noted that the deconstruction and waste
No packaging waste is landfilled. treatment scenario can vary a lot, depending on the actual
The use of multi-way pallets is not taken into account as situation. Thus, a generic end-of-life scenario is assumed.
packaging material.
As a rule of thumb, metals are recycled, plastics are incinerated
Reference service life (also due to the very limited availability on plastics recycling
Name Value Unit and its benefits); coated and uncoated flat glass is assumed to
be recycled whereas laminated glass is assumed to be
Reference service life
landfilled due to very limited recycling potential.
according to 30 a
manufacturer's declaration
The combustible material (mainly plastics) is assumed to be
The product has passed
Declared product transported 50 km with a lorry 16-32 metric tons, EURO6 to an
internal quality controls and
properties (at the gate) and - incineration plant.
complies with EN 1873 for CE
finishes
marking
Metals and flat glass recycled; it is assumed that these fractions
Design application reach the end-of-waste state after having been sorted and
parameters (if instructed by transported to a recycler over 150 km with a lorry 16-32 metric
Installation according to
the manufacturer), tons, EURO6.
assembly instructions and -
including the references to
state of the art.
the appropriate practices Laminated glass is landfilled, including a transport of 30 km with
and application codes a lorry 16-32 metric tons, EURO6.
An assumed quality of
Carried out in accordance
work, when installed in Module C3
with the manufacturer's -
accordance with the A consumption of 0.03 kWh/kg of electricity for shredding and
instructions.
manufacturer’s instructions sorting and 0.437 MJ/kg of diesel fuel for internal logistics are
Outdoor environment, (for The declared products are taken into account to disassemble the product. The recovered
outdoor applications), e.g. intended for installation material leaves the product system as 'materials for recycling'.
weathering, pollutants, UV outside the building: They are The net amounts of the metals leaving the product system are
and wind exposure, therefore designed to - considered as 'use of secondary material' in Module D.
building orientation, withstand outdoor conditions
shading, temperature throughout their service life. Module C4
As stated above, it is assumed that 100 % of the plastic parts
Indoor environment (for
The declared products are and the wooden parts are treated in a waste incineration plant
indoor applications), e.g.
not intended for installation - with an efficiency R1 < 0.6 (according to the ecoinvent dataset
temperature, moisture,
inside a building. used); 25.57 % of the lower heating value of the plastic parts
chemical exposure
are recovered as heat and 13.0 % as electricity. Recovered
Usage conditions, e.g. Standard use in any type of
energy is reported as 'exported energy' and considered in
frequency of use, building, i.e. opening/closing -
Module D.
mechanical exposure as often as necessary.
The declared products are Some of the material, notably laminated flat glass is assumed
Maintenance e.g. required designed for a reference life to be landfilled.
frequency, type and quality of 30 years. They are
-
and replacement of maintained by cleaning water Module D
components at the discretion of the Module D contains the benefits and loads beyond the system
building occupants. boundary related to the recycling of metals, which result from
Module B1 the treatment of recycled materials from the point of end-of-
The products are assumed to have no direct emissions during waste status to the point of substitution (as loads) and the
the use phase. The indicator values of Module B1 are thus 0. substitution of primary resources (as benefits).
For biogenic carbon storage, see table above.
Furthermore, it includes the benefits of raw material substitution
Module B2 of the recycling of flat glass, with the exception of laminated
For fixed flat roof windows, no impacts related to maintenance glass, which cannot be used for the production of glass again.
are inventoried in module B2. Annual cleaning with water (e.g., Recovered flat glass is assumed to have reached the end-of-
using 1 l/m2 of tap water per annual cleaning) is neglected. waste state as sorted glass cullet; glass cullet is assumed to
replace virgin raw material for glass production – impacts on
the energy required to remelt recycled glass as compared to
Module B6
virgin glass production are neglected due to a lack of data.
Fixed flat roof windows do not consume operational energy.
It also includes the benefits and loads related to the energy
Module C1
recovery from plastic wastes in a MWIP as modelled in
Manual de-installation is assumed, electricity consumption
Modules A3, A5 and C3.
related to electric screw drivers, etc. is considered to be
negligible. Thus, no environmental impacts are declared in
Due to a lack of data for plastics from de-construction activities,
module C1.
the substitution potential of recycled plastics is not taken into
account.
Module C2
Given the complexity of the inventoried products, a mixed end-
Only net flows leaving the product system are considered in
5 Environmental Product Declaration - VELUX A/S - VELUX flat roof window CFP
module D.
6 Environmental Product Declaration - VELUX A/S - VELUX flat roof window CFP
5. LCA: Results
Disclaimer:
EP-freshwater: This indicator has been calculated as 'kg P eq' as required in the characterization model (EUTREND model, Struijs et
al., 2009b, as implemented in ReCiPe; http://eplca.jrc.ec.europa.eu/LCDN/developerEF.xhtml)
DESCRIPTION OF THE SYSTEM BOUNDARY (X = INCLUDED IN LCA; MND = MODULE OR INDICATOR NOT DECLARED; MNR
= MODULE NOT RELEVANT)
Benefits and
Construction loads beyond
Product stage Use stage End of life stage
process stage the system
boundaries
la ire ta m w a Ry lp p u s tro p s n a rT g n iru tc a fu n a M e h t m o rf tro p s n a rTe tis e h t o t e ta g y lb m e s s A e s U e c n a n e tn ia M ria p e R tn e m e c a lp e R tn e m h s ib ru fe R y g re n e la n o ita re p Oe s u re ta w la n o ita re p Oe s u n o itc u rts n o c -e Dn o itilo m e d tro p s n a rT g n is s e c o rp e ts a W la s o p s iD -e s u e R-y re v o c e R-g n ilc y c e Rla itn e to p
A1 A2 A3 A4 A5 B1 B2 B3 B4 B5 B6 B7 C1 C2 C3 C4 D
X X X MND X X X MNR MNR MNR X MND X X X X X
RESULTS OF THE LCA - ENVIRONMENTAL IMPACT according to EN 15804+A2: 1 piece VELUX flat roof window CFP with a
fixed base unit, 1.20 m x 1.20 m = 1.44 m2
Parameter Unit A1-A3 A5 B1 B2 B6 C1 C2 C3 C4 D
GWP-total kg CO 2 eq 1.83E+02 8.9E+00 0 0 0 0 3.69E-01 1.47E+00 8.05E+01 -3.01E+01
GWP-fossil kg CO 2 eq 1.9E+02 1.85E+00 0 0 0 0 3.69E-01 1.38E+00 8.05E+01 -3.01E+01
GWP-
biogenic kg CO 2 eq -7.13E+00 7.04E+00 0 0 0 0 0 9.06E-02 0 0
GWP-luluc kg CO 2 eq 1.41E-01 8.38E-05 0 0 0 0 1.5E-04 1.54E-03 2.6E-02 -2.27E-02
ODP kg CFC11 eq 5.02E-05 4.74E-08 0 0 0 0 8.65E-08 8.5E-08 8.9E-06 -2.44E-06
AP mol H+ eq 7.64E-01 1.3E-03 0 0 0 0 2.09E-03 5.27E-03 9.88E-02 -4.96E-02
EP-
kg P eq 4.78E-03 1.6E-06 0 0 0 0 2.71E-06 1.79E-04 7.71E-04 -2.6E-03
freshwater
EP-marine kg N eq 1.41E-01 4.87E-04 0 0 0 0 7.51E-04 1.69E-03 2.21E-02 -9.84E-03
EP-terrestrial mol N eq 1.52E+00 5.39E-03 0 0 0 0 8.27E-03 1.92E-02 2.43E-01 -1.18E-01
kg NMVOC
POCP 4.79E-01 1.52E-03 0 0 0 0 2.36E-03 5.12E-03 6.53E-02 -3.35E-02
eq
ADPE kg Sb eq 5.38E+02 6.94E-07 0 0 0 0 1.23E-06 2.4E-06 2.06E-04 -5.09E-05
ADPF MJ 2.61E+03 3.11E+00 0 0 0 0 5.67E+00 1.91E+01 2E+02 -4.57E+02
m3 world eq
WDP 7.07E+01 1.26E-02 0 0 0 0 1.86E-02 4.75E-02 1.47E+01 -8.29E-01
deprived
GWP = Global warming potential; ODP = Depletion potential of the stratospheric ozone layer; AP = Acidification potential of land and water; EP =
Eutrophication potential; POCP = Formation potential of tropospheric ozone photochemical oxidants; ADPE = Abiotic depletion potential for non-fossil
resources; ADPF = Abiotic depletion potential for fossil resources; WDP = Water (user) deprivation potential)
RESULTS OF THE LCA - INDICATORS TO DESCRIBE RESOURCE USE according to EN 15804+A2: 1 piece VELUX flat roof
window CFP with a fixed base unit, 1.20 m x 1.20 m = 1.44 m2
Parameter Unit A1-A3 A5 B1 B2 B6 C1 C2 C3 C4 D
PERE MJ 1.09E+02 4.71E-02 0 0 0 0 8.02E-02 2.41E+00 2.23E+01 -3.62E+01
PERM MJ 8.2E+01 -8.09E+01 0 0 0 0 0 -1.17E+00 0 0
PERT MJ 1.91E+02 -8.08E+01 0 0 0 0 8.02E-02 1.24E+00 2.23E+01 -3.62E+01
PENRE MJ 2.5E+03 2.83E+01 0 0 0 0 5.68E+00 1.52E-05 9.64E+02 -4.63E+02
PENRM MJ 7.9E+02 -2.52E+01 0 0 0 0 0 0 -7.64E+02 0
PENRT MJ 3.29E+03 3.11E+00 0 0 0 0 5.68E+00 1.52E-05 2E+02 -4.63E+02
SM kg 7.63E+00 0 0 0 0 0 0 0 0 -1.19E+01
RSF MJ 0 0 0 0 0 0 0 0 0 0
NRSF MJ 0 0 0 0 0 0 0 0 0 0
FW m3 1.59E+00 6.18E-04 0 0 0 0 6.18E-04 4.55E-03 3.84E-01 -6.89E-02
PERE = Use of renewable primary energy excluding renewable primary energy resources used as raw materials; PERM = Use of renewable primary
energy resources used as raw materials; PERT = Total use of renewable primary energy resources; PENRE = Use of non-renewable primary energy
excluding non-renewable primary energy resources used as raw materials; PENRM = Use of non-renewable primary energy resources used as raw
materials; PENRT = Total use of non-renewable primary energy resources; SM = Use of secondary material; RSF = Use of renewable secondary fuels;
NRSF = Use of non-renewable secondary fuels; FW = Use of net fresh water
RESULTS OF THE LCA – WASTE CATEGORIES AND OUTPUT FLOWS according to EN 15804+A2:
1 piece VELUX flat roof window CFP with a fixed base unit, 1.20 m x 1.20 m = 1.44 m2
Parameter Unit A1-A3 A5 B1 B2 B6 C1 C2 C3 C4 D
HWD kg 8.24E-03 8.19E-06 0 0 0 0 1.45E-05 1.52E-05 3.4E-04 -3.91E-04
NHWD kg 2.52E+01 2.23E-01 0 0 0 0 3.8E-01 7.76E-02 3.66E+01 -1.81E+00
7 Environmental Product Declaration - VELUX A/S - VELUX flat roof window CFP
RWD kg 1.65E-02 4.42E-05 0 0 0 0 8.2E-05 1.72E-04 1.52E-03 -2.01E-03
CRU kg 0 0 0 0 0 0 0 0 0 0
MFR kg 5.15E+00 4.82E+00 0 0 0 0 0 1.03E+00 0 0
MER kg 0 0 0 0 0 0 0 0 0 0
EEE MJ 1.09E+00 3.28E+00 0 0 0 0 0 0 9.94E+01 0
EET MJ 2.05E+00 6.45E+00 0 0 0 0 0 0 1.95E+02 0
HWD = Hazardous waste disposed; NHWD = Non-hazardous waste disposed; RWD = Radioactive waste disposed; CRU = Components for re-use;
MFR = Materials for recycling; MER = Materials for energy recovery; EEE = Exported electrical energy; EET = Exported thermal energy
RESULTS OF THE LCA – additional impact categories according to EN 15804+A2-optional:
1 piece VELUX flat roof window CFP with a fixed base unit, 1.20 m x 1.20 m = 1.44 m2
Parameter Unit A1-A3 A5 B1 B2 B6 C1 C2 C3 C4 D
Disease
PM 5.04E-06 1.92E-08 0 0 0 0 3.32E-08 8.18E-08 7.65E-07 -1.89E-07
incidence
IR kBq U235 eq 4.37E+00 1.34E-02 0 0 0 0 2.46E-02 6.62E-02 8.66E-01 -8.31E-01
ETP-fw CTUe 2.93E+03 3.25E+00 0 0 0 0 4.49E+00 1.12E+01 3.73E+03 -1.64E+02
HTP-c CTUh 1.22E-07 2.99E-10 0 0 0 0 1.79E-10 3.03E-10 2.5E-08 -1.13E-08
HTP-nc CTUh 2.1E-06 4.32E-09 0 0 0 0 5.17E-09 9.86E-09 9.43E-07 -1.04E-07
SQP SQP 6.15E+02 2.62E+00 0 0 0 0 4.84E+00 2.58E+00 6.63E+01 -3.64E+01
PM = Potential incidence of disease due to PM emissions; IR = Potential Human exposure efficiency relative to U235; ETP-fw = Potential comparative
Toxic Unit for ecosystems; HTP-c = Potential comparative Toxic Unit for humans (cancerogenic); HTP-nc = Potential comparative Toxic Unit for humans
(not cancerogenic); SQP = Potential soil quality index
Disclaimer 1 – for the indicator 'Potential Human exposure efficiency relative to U235'.This impact category deals mainly with the
eventual impact of low-dose ionizing radiation on human health of the nuclear fuel cycle. It does not consider effects due to possible
nuclear accidents, occupational exposure or radioactive waste disposal in underground facilities. Potential ionizing radiation from the
soil, radon and from some construction materials is also not measured by this indicator.
Disclaimer 2 – for the indicators 'abiotic depletion potential for non-fossil resources', 'abiotic depletion potential for fossil resources',
'water (user) deprivation potential, deprivation-weighted water consumption', 'potential comparative toxic unit for ecosystems', 'potential
comparative toxic unit for humans – cancerogenic', 'Potential comparative toxic unit for humans - not cancerogenic', 'potential soil
quality index'. The results of this environmental impact indicator shall be used with care as the uncertainties on these results are high
as there is limited experience with the indicator.
6. LCA: Interpretation
Figure 1 illustrates the relative contributions of the different
modules along the life cycle of the declared products.
are in the order of 0 % to 45% of the impacts over the product
life cycle (modules A1-C4). [1]
Figure1: Relative environmental impacts of the different life
cycle stages for the flat roof window CFP fixed The use of renewable primary energy is mainly caused by the
share of renewable energy in the electricity mix, thus the
The largest part of environmental impacts – between 65 % and production stage is the main driver of this impact category; also
rather100 % - is caused during production (modules A1-A3) of for the use of non-renewable primary energy, the production
the flat roof window. No operational energy is used as the flat phase is the most impacting life cycle stage.
roof window cannot be opened.
Material use of primary energy is negligible and related to
Benefits and burdens beyond the system boundary (module D) plastic parts of the product and packaging material. The
8 Environmental Product Declaration - VELUX A/S - VELUX flat roof window CFP
material use of primary energy is transferred to its energy use wastes are mainly caused by the European electricity mix.
when the materials containing primary energy are incinerated
with energy recovery. [1] Benefits resulting from the recycling of plastics as well as
from the recycling of the electronic parts are disregarded due to
Non-hazardous waste as the quantitatively most relevant waste the lack of data on the recycling processes and related to the
flows is mainly caused during the production of the glass and detailed composition of the electronic parts.
during disposal of the product; hazardous and radio-active
7. Requisite evidence
to AltholzVO
8.1 Formaldehyde Not applicable; not tested based on applicable product
Not tested based on applicable product standard. standard. 7.4. Fire gas toxicity
Not tested based on applicable product standard. 7.5 VOC
7.2 MDI emissions
Not tested based on applicable product standard. 7.3 Not tested based on applicable product standard.
Checking of pre-treatment of substances used according
8. References
Product category rules of IBU DIN EN 1873:2005, Prefabricated accessories for roofing -
Individual rooflights of plastics - Product specification and test
IBU (2021) methods.
IBU (2021): General Instructions for the EPD Programme of the
Institut Bauen & Umwelt e.V. (General Instructions for the IBU EN 16485
EPD Programme). Version 2.0, Institut Bauen & Umwelt, Berlin DIN EN 16485:2014-07, Round and sawn timber -
Environmental Product Declarations - Product category rules
IBU (2017) for wood and wood-based products for use in construction;
IBU (2017): PCR Teil A: PCR Part A: Calculation rules for the German version EN 16485:2014.
life cycle assessment and requirements for the project report.
Version 1.8., Institut Bauen & Umwelt, Berlin. ECHA-List
The Candidate List of substances of very high concern,
IBU (2021) available via https://echa.europa.eu/nl/-/four-newsubstances-
IBU (2021):PCR Part B: Requirements on the EPD for windows added-to-the-candidate-list.
and doors. Version 2021/01, Institut Bauen & Umwelt, Berlin.
Regulation on biocidal products
Standards and legal documents REGULATION (EU) No 528/2012 OF THE EUROPEAN
PARLIAMENT AND OF THE COUNCIL of 22 May 2012
EN 15804 concerning the making available on the market and use of
DIN EN 15804+A2:2019, Sustainability of construction works - biocidal products.
Environmental product declarations - Core rules for the product
category construction products. Regulation (EU) Nr. 305/2011(CPR)
REGULATION (EU) No 305/2011 OF THE EUROPEAN
ISO 14025 PARLIAMENT AND OF THE COUNCIL of 9 March 2011 laying
DIN EN ISO 14025:2006-07, Environmental labels and down harmonised conditions for the marketing of construction
declarations - Type III Environmental declarations - Principles products and repealing Council Directive 89/106/EEC.
and procedures.
COUNCIL REGULATION (EU) No 333/2011
ISO 14044 COUNCIL REGULATION (EU) No 333/2011 of 31 March 2011
DIN EN ISO 14044:2006-07, Environmental management - Life establishing criteria determining when certain types of scrap
cycle assessment - Requirements and guidance (ISO metal cease to be waste under Directive 2008/98/EC of the
14044:2006); German and English versions EN ISO European Parliament and of the Council.
14044:2006.
European Waste List (Waste index)
ISO 9001 http://www.gesetze-im-internet.de/avv/anlage.htm
DIN EN ISO 9001:2015, Quality management systems -
Requirements. Additional references
ISO 14001 Weidema et al. (2013)
DIN EN ISO 14001:2015: Environmental management Weidema, B., C. Bauer, R. Hischier, C. Mutel, T. Nemecek, J.
systems - Requirements with guidance for use. Reinhard, C.O. Vadenbo, G. Wernet (2013): Overview and
methodology, Data quality guideline for the ecoinvent database
ISO 45001 version 3. ecoinvent report no. 1 (v3), St. Gallen, Schweiz.
ISO 45001:2018-03, Occupational health and safety
management systems - Requirements with guidance for use. ecoinvent 3.8
ecoinvent 3.8, LCA database, 12/2021. Ecoinvent centre,
EN 1873 Zürich.
9 Environmental Product Declaration - VELUX A/S - VELUX flat roof window CFP
Publisher
Institut Bauen und Umwelt e.V. +49 (0)30 3087748- 0
Hegelplatz 1 info@ibu-epd.com
10117 Berlin www.ibu-epd.com
Germany
Programme holder
Institut Bauen und Umwelt e.V. +49 (0)30 3087748- 0
Hegelplatz 1 info@ibu-epd.com
10117 Berlin www.ibu-epd.com
Germany
Author of the Life Cycle Assessment
Dr. Frank Werner - Umwelt & Entwicklung + 41 (0)44 241 39 06
Kammelenbergstrasse 30 frank@frankwerner.ch
9011 St. Gallen http://www.frankwerner.ch/
Switzerland
Owner of the Declaration
VELUX Group +4545164726
Ådalsvej 99 jakob.roerbech@velux.com
2970 Hørsholm www.velux.com
Denmark
10 Environmental Product Declaration - VELUX A/S - VELUX flat roof window CFP
