ENVIRONMENTAL PRODUCT DECLARATION
as per ISO 14025 and EN 15804+A2
Owner of the Declaration Give Steel A/S
Publisher Institut Bauen und Umwelt e.V. (IBU)
Programme holder Institut Bauen und Umwelt e.V. (IBU)
Declaration number EPD-GIV-20220239-IBA1-EN
Issue date 31/08/2023
Valid to 30/08/2028
Galvanized Structural Steel
Give Steel A/S
www.ibu-epd.com | https://epd-online.com
1. General Information
Give Steel A/S Galvanized Structural Steel
Programme holder Owner of the declaration
IBU – Institut Bauen und Umwelt e.V. Give Steel A/S
Hegelplatz 1 Sjællandsvej 14
10117 Berlin 7330 Brande
Germany Denmark
Declaration number Declared product / declared unit
EPD­GIV­20220239­IBA1­EN 1 t of galvanized structural steel.
This declaration is based on the product category rules: Scope:
Structural steels, 01/08/2021 The declaration covers galvanized structural steel produced at the
(PCR checked and approved by the SVR) production site in Brande, Denmark. The declaration covers all life cycle
modules from A1­A5, C1­C4 and D and is based on product­specific data
provided by Give Steel A/S and background data from GaBi professional
Issue date 2020 and Ecoinvent v3.6.
The owner of the declaration shall be liable for the underlying information
31/08/2023
and evidence; the IBU shall not be liable with respect to manufacturer
information, life cycle assessment data and evidences.
Valid to
The EPD was created according to the specifications of EN 15804+A2. In
30/08/2028 the following, the standard will be simplified as EN 15804.
Verification
The standard EN 15804 serves as the core PCR
Independent verification of the declaration and data according to ISO
14025:2011
internally X externally
Dipl.­Ing. Hans Peters
(Chairman of Institut Bauen und Umwelt e.V.)
Florian Pronold Mrs Kim Allbury,
(Managing Director Institut Bauen und Umwelt e.V.) (Independent verifier)
1 Environmental Product Declaration ­ Give Steel A/S ­ Galvanized Structural Steel
2. Product
Name Value Unit
2.1 Product description/Product definition
Scrap steel 78 %
This EPD applies to 1 ton of galvanized structural steel.
Primary steel 20 %
Structural steel constructions from Give Steel are designed and
produced according to European design codes and production Welding rod (iron) 1 %
standards, as well as in compliance with project specifications. Galvanization (zinc) 1 %
While Eurocode 1 and Eurocode 3 apply to the design and civil
The product constitutes primarily of steel scrap (78 %) and
engineering works, manufacturing is carried out according to
primary steel (20 %). Welding rod (iron) and galvanization (zinc)
EN 1090 for steel construction.
account for 1 % respectively.
The galvanized structural steel does not contain substances
Furthermore, these codes and standards outline specific
listed in the 'Candidate List of Substances of Very High
product standards for choosing the most appropriate constitute
Concern for Authorisation' (SVHC).
products for each component. Such standards include EN
10025 which defines the requirements for non­alloy and fine
This product/article/at least one partial article contains
grain weldable structural steels, EN 10219 for cold formed
substances listed in the candidate list (date: 23.05.2023)
hollow sections and EN 13479 and ISO 544 which sets out the
exceeding 0.1 percentage by mass: No
same set of requirements for materials. For the placing on the
market of the product in the European Union/European Free
This product/article/at least one partial article contains other
Trade Association (EU/EFTA) (with the exception of
carcinogenic, mutagenic, reprotoxic (CMR) substances in
Switzerland) Regulation (EU) No. 305/2011 (CPR) applies. The
categories 1A or 1B which are not on the candidate list,
product needs a declaration of performance taking into
exceeding 0.1 percentage by mass: No
consideration EN 10025­1:2004 Hot rolled products of
structural steels – Part 1: General technical delivery conditions
Biocide products were added to this construction product or it
and the CE­marking.
has been treated with biocide products (this then concerns a
2.2 Application treated product as defined by the (EU) Ordinance on Biocide
Products No. 528/2012): No
The product can be used as part elements or as an
independent static system, where all parts are made of steel.
2.6 Manufacture
The product is widely used in numerous construction projects.
The product stage comprises the acquisition of all raw
Examples are:
materials, products and energy, transport to the production site,
• Single­story buildings (industrial and storage halls, packaging and waste processing up to the ”end­of­waste” state
animal stables, data centres, etc.) or final disposal. The LCA results are declared in aggregated
• Multi­story buildings (offices, residential buildings, car form for the product stage, which means that the sub­modules
parks, etc.) A1, A2 and A3 are declared as one module A1­A3.
• Bridges (railway bridge, road bridge, pedestrian bridge,
etc.) The raw materials: flat iron, plate and beams are brought in,
• Other structures (Stadiums, convention centres, processed, shot cleaned, cut and welded. The process will vary,
airports, stations, etc.) depending on the involved raw material.
2.3 Technical Data
The various materials are transported by side loader from our
This EPD is valid for galvanized structural steel of different warehouse to the appropriate production machines: Flat iron to
forms of delivery. Specific information on dimension tolerances, the computerized numerical control (CNC) flat iron machine,
constructional data as well as mechanical and chemical plate to the CNC plasma cutter and beams to the shot ball
properties can be found in the relevant literature and/or the cleaner. Flat iron is processed if necessary, by adding holes
standards. and cutting into strips. Plate is plasma cut following 2D models.
Constructional data Beams are shot cleaned and cut to length. Flat iron, steel plate
and beams are shot cleaned before production to produce the
Name Value Unit
correct surface. The shot cleaner is always kept full to save
Density 7850 kg/m3
power. The steel balls are reused in production until steel dust
Modulus of elasticity 210000 N/mm2 is all that remains. After cleaning, the flat iron and plate are
Coefficient of thermal expansion 12 10­6K­1 distributed for use as beams and to the welding robot,
respectively. Beams and associated plates are stapled together.
Thermal conductivity 48 W/(mK)
Beams are then welded, according to design diagrams.
Melting point 1536 °C
Performance data of the product in accordance with the When manufacturing welded wedges for robot welding, all parts
declaration of performance with respect to its essential are assembled from the CNC cutting table and CNC flat iron
characteristics according to EN 10025, Hot­rolled products of cutter. Once the parts are collected they are stapled together
structural steels. according to design diagrams. The stapled wedges are robot
welded and sent on. The remaining components are mounted
2.4 Delivery status or welded manually.
The dimensions of the product declared in this EPD may vary
depending on the intended application. Beams that need to be galvanized are loaded onto a lorry and
transported to a subcontractor. After galvanization, the beams
2.5 Base materials/Ancillary materials
are brought back to the factory and stored until delivery to the
Material composition construction site.
2.7 Environment and health during manufacturing
2 Environmental Product Declaration ­ Give Steel A/S ­ Galvanized Structural Steel
During the entire manufacturing process, no other health material does not emit fumes or fire gases.
protection measures are required extending beyond the legally
Fire protection
specified industrial protection measures for commercial
Name Value
enterprises.
Building material class according to EN 13501­1 A1
2.8 Product processing/Installation
The product is installed using a diesel truck. No auxiliary
Water
materials are used.
Steel is stable in water, insoluble and does not emit substances
in water. In case of flooding, no impacts are to be
2.9 Packaging
expected. Steel can corrode in the presence of oxygen in the
The product is delivered with metal strips and cardboard as
water (= slow oxidation).
packaging.
2.10 Condition of use Mechanical destruction
Steel components display very good characteristics when
During use, no changes in material composition shall occur.
exposed to extraordinary mechanical impact. As a general rule,
The product does not require maintenance.
no chips, breaking edges or similar are incurred.
2.11 Environment and health during use
2.14 Re-use phase
Under normal use conditions, structural steel products do not
The product has a 100 % recycling potential.
cause any adverse health effects nor release other emissions
to indoor air. Also, no environmental impacts on water, air or
2.15 Disposal
soil are expected.
Due to its high value as a resource, steel scrap is not disposed
2.12 Reference service life of but instead fed into a well­established cycle
of reuse or recycling. However, in the case of dumping due to
A reference service life for structural steel is not declared. It is a
collection loss, no environmental impacts are
construction product with many different application purposes.
expected. Waste code in accordance with the European Waste
The lifetime therefore will be limited by the service life of the
Catalogue (EWC): (17 04 05 Iron and steel).
work. The same applies for aging.
2.16 Further information
2.13 Extraordinary effects
Further information on the product can be obtained from
Fire
givesteel.com.
The material is class A1, i.e. not flammable per EN 13501. The
3. LCA: Calculation rules
3.1 Declared Unit 3.3 Estimates and assumptions
The declared unit is 1 ton of galvanized structural steel. The It is assumed that 100 % of the product can be recycled,
galvanization accounts for 1 % of the product's weight­%. though 5 % of the product is lost at recycling. The recycling of
the product is assumed to replace scrap steel in module D.
Declared unit
Name Value Unit 3.4 Cut-off criteria
Declared unit 1 t The declaration covers all relevant processes and aspects of
Density 7850 kg/m3 the life cycle for galvanized structural steel. Only the production
of capital goods, buildings and equipment during the production
The conversion factor to 1 kg is 0.001.
of steel in A1 has been omitted from the LCA study, as it is
assumed to be negligible.
3.2 System boundary
Thus, the declaration is in compliance with the rules in EN
Type of EPD: Cradle to gate with options.
15804, 6.3.5, where the omission for input­flows per module
Module A1­A3, A4, A5, B1­B7, C1­C4 and D are considered.
must be a maximum 5 % of energy usage and mass and at
Yet, no environmental impacts are associated with modules B1­
most 1 % for unit processes.
B7, thus these modules are declared as 'not relevant' or 'not
declared'. 3.5 Background data
The LCA model is developed using GaBi Software developed
Modules A1-A3 include the acquisition of all raw materials,
by Sphera Solutions GmbH. The databases, GaBi Professional
products and energy, transport to the production site, the
2020 and EcoInvent 3.6, provide the life cycle inventory data
manufacturing of the galvanized structural steel and waste
used from the background system.
processing up to the 'end­of­waste' state.
3.6 Data quality
Module A4 includes the transport of the product to the The product­specific data have been collected by Give Steel
construction site. A/S and are based on the yearly production amounts and
Module A5 includes the installation of the product using a energy consumption at the production site located in Brande,
diesel truck. Denmark in 2019. Background data are based on GaBi
Professional and EcoInvent 3.6 and are less than 10 years old.
Module C1 considers the deconstruction of the structural steel Generally, the used background datasets are of good quality,
using a truck. In module C2, the demolished steel is and the majority of the datasets are only a couple of years old.
transported to a waste processing site, with the waste
processing considered in module C3. 3.7 Period under review
The foreground data was collected by Give Steel A/S in the
Finally, module D considers the benefits from recycling the period January 2019 to December 2019. The declaration is
demolished steel parts. therefore based on average values for the production amount
3 Environmental Product Declaration ­ Give Steel A/S ­ Galvanized Structural Steel
from the year 2019. consumption at the production site is allocated through mass
allocation.
3.8 Geographic Representativeness
Land or region, in which the declared product system is 3.10 Comparability
manufactured, used or handled at the end of the product´s Basically, a comparison or an evaluation of EPD data is only
lifespan: Europe possible if all the data sets to be compared were created
according to EN 15804 and the building context, respectively
the product­specific characteristics of performance, are taken
3.9 Allocation
into account. Background data was mainly taken from GaBi
The allocation is made in accordance with the provisions of EN Professional 2020. Ecoinvent 3.6 was used whendatasets were
15804. A conservative approach is used for the allocation not available in GaBi Professional2020.
of by­products in steel manufacturing, meaning that all impact is
attributed to the main product of steel. Energy, heat and water
4. LCA: Scenarios and additional technical information
A diesel truck is used to install the product. Based on annual
Characteristic product properties of biogenic carbon data from Give Steel A/S, 0.261 kg diesel is used for the
The product does not contain any biogenic carbon. The installation of 1 ton of galvanized structural steel.
packaging includes a small amount of biogenic carbon, as
Name Value Unit
cardboard is used as packaging.
Other resources Diesel 0.261 kg
Note: 1 kg biogenic carbon is equivalent to 44/12 kg of CO Use stage (B1-B7)
2
There are no environmental impacts associated with the use
Information on describing the biogenic Carbon Content at
stage (B1­B7).
factory gate
Name ValueUnit Reference service life
kg The reference service life of the product depends on its
Biogenic carbon content in product 0 ­
C application.
Biogenic carbon content in accompanying kg
0.012
packaging 0 C A reference service life for structural steel is not declared.
End of life (C1 - C4)
A conservative distance of 300 km is used in module A4. Name Value Unit
Transport to the building site (A4) Collected separately structural steel 1000 kg
Name Value Unit Collected as mixed construction waste ­ kg
Litres of fuel 2.7 l/100km Reuse ­ kg
Transport distance 300 km Recycling 1000 kg
Capacity utilisation (including empty runs) 85 % Energy recovery ­ kg
Gross density of products transported 7850 kg/m3 Landfilling ­ kg
Capacity utilisation volume factor 0.55 ­ Reuse, recovery and/or recycling potentials (D), relevant
scenario information
Installation into the building (A5) The product has a 100 % recycling potential, yet, 5 % of the
product is assumed to be lost through the recycling process.
4 Environmental Product Declaration ­ Give Steel A/S ­ Galvanized Structural Steel
5. LCA: Results
The LCA results cover modules A1­A5, C1­C4 and D. No environmental impacts are associated with modules B1­B7; thus, these
modules are marked as 'not relevant' or 'not declared' in the table below.
DESCRIPTION OF THE SYSTEM BOUNDARY (X = INCLUDED IN LCA; ND = MODULE OR INDICATOR NOT DECLARED; MNR =
MODULE NOT RELEVANT)
Benefits and
Construction loads beyond
Product stage Use stage End­of­life stage
process stage the system
boundaries
la ire ta m w a Ry lp p u s tro p s n a rT g n iru tc a fu n a M e h t m o rf tro p s n a rTe tis e h t o t e ta g y lb m e s s A e s U e c n a n e tn ia M ria p e R tn e m e c a lp e R tn e m h s ib ru fe R y g re n e la n o ita re p Oe s u re ta w la n o ita re p Oe s u n o itc u rts n o c ­e Dn o itilo m e d tro p s n a rT g n is s e c o rp e ts a W la s o p s iD ­e s u e R­y re v o c e R­g n ilc y c e Rla itn e to p
A1 A2 A3 A4 A5 B1 B2 B3 B4 B5 B6 B7 C1 C2 C3 C4 D
X X X X X MND MND MNR MNR MNR MND MND X X X X X
RESULTS OF THE LCA - ENVIRONMENTAL IMPACT according to EN 15804+A2: 1 ton galvanized structural steel
Parameter Unit A1-A3 A4 A5 C1 C2 C3 C4 D
GWP­total kg CO 2 eq 1.04E+03 8.39E+00 6.58E­01 6.58E­01 8.47E+00 2.33E+01 0 ­3.16E+02
GWP­fossil kg CO 2 eq 1.03E+03 8.23E+00 6.93E­01 6.93E­01 8.32E+00 2.47E+01 0 ­3.15E+02
GWP­biogenic kg CO 2 eq 2.94E+00 8.95E­02 0 0 9.04E­02 0 0 ­2.04E­01
GWP­luluc kg CO 2 eq 1.26E+00 6.74E­02 7.62E­03 7.62E­03 6.8E­02 2.81E­02 0 4.56E­02
ODP kg CFC11 eq 8.63E­12 1.53E­15 1.73E­16 1.73E­16 1.54E­15 3.54E­06 0 ­5.26E­13
AP mol H+ eq 2.99E+00 3E­02 3.41E­03 3.41E­03 3.03E­02 2.99E­01 0 ­5.66E­01
EP­freshwater kg P eq 1.66E­03 2.54E­05 2.87E­06 2.87E­06 2.56E­05 2.09E­02 0 ­6.45E­05
EP­marine kg N eq 8.43E­01 1.37E­02 1.52E­03 1.52E­03 1.38E­02 6.79E­02 0 ­8.44E­02
EP­terrestrial mol N eq 9.17E+00 1.53E­01 1.69E­02 1.69E­02 1.54E­01 7.66E­01 0 ­8.23E­01
kg NMVOC
POCP 2.56E+00 2.67E­02 4.29E­03 4.29E­03 2.7E­02 2.09E­01 0 ­4.32E­01
eq
ADPE kg Sb eq 2.94E­04 6.73E­07 7.61E­08 7.61E­08 6.8E­07 1.37E­03 0 ­6.86E­04
ADPF MJ 1.12E+04 1.11E+02 1.26E+01 1.26E+01 1.12E+02 3.7E+02 0 ­2.74E+03
m3 world eq
WDP 1.46E+01 8.12E­02 9.18E­03 9.18E­03 8.2E­02 6.97E+00 0 ­6.19E+01
deprived
GWP = Global warming potential; ODP = Depletion potential of the stratospheric ozone layer; AP = Acidification potential of land and water; EP =
Eutrophication potential; POCP = Formation potential of tropospheric ozone photochemical oxidants; ADPE = Abiotic depletion potential for non­fossil
resources; ADPF = Abiotic depletion potential for fossil resources; WDP = Water (user) deprivation potential)
RESULTS OF THE LCA - INDICATORS TO DESCRIBE RESOURCE USE according to EN 15804+A2: 1 ton galvanized structural
steel
Parameter Unit A1-A3 A4 A5 C1 C2 C3 C4 D
PERE MJ 2.14E+03 6.42E+00 7.26E­01 7.26E­01 6.49E+00 5.37E+01 0 2.52E+02
PERM MJ 5.88E­02 0 0 0 0 0 0 0
PERT MJ 2.14E+03 6.42E+00 7.26E­01 7.26E­01 6.49E+00 5.37E+01 0 2.52E+02
PENRE MJ 1.13E+04 1.11E+02 1.26E+01 1.26E+01 1.13E+02 3.7E+02 0 ­2.75E+03
PENRM MJ 0 0 0 0 0 0 0 0
PENRT MJ 1.13E+04 1.11E+02 1.26E+01 1.26E+01 1.13E+02 3.7E+02 0 ­2.75E+03
SM kg 7.84E+02 0 0 0 0 0 0 0
RSF MJ 0 0 0 0 0 0 0 0
NRSF MJ 0 0 0 0 0 0 0 0
FW m3 2.14E+00 7.48E­03 8.46E­04 8.46E­04 7.56E­03 1.62E­01 0 ­1.39E+00
PERE = Use of renewable primary energy excluding renewable primary energy resources used as raw materials; PERM = Use of renewable primary
energy resources used as raw materials; PERT = Total use of renewable primary energy resources; PENRE = Use of non­renewable primary energy
excluding non­renewable primary energy resources used as raw materials; PENRM = Use of non­renewable primary energy resources used as raw
materials; PENRT = Total use of non­renewable primary energy resources; SM = Use of secondary material; RSF = Use of renewable secondary fuels;
NRSF = Use of non­renewable secondary fuels; FW = Use of net fresh water
RESULTS OF THE LCA – WASTE CATEGORIES AND OUTPUT FLOWS according to EN 15804+A2:
1 ton galvanized structural steel
Parameter Unit A1-A3 A4 A5 C1 C2 C3 C4 D
HWD kg 3.85E­05 5.16E­06 5.83E­07 5.83E­07 5.21E­06 0 0 7.66E­07
NHWD kg 1.09E+01 1.77E­02 2E­03 2E­03 1.78E­02 0 0 3.3E+01
RWD kg 2.96E­01 2.06E­04 2.32E­05 2.32E­05 2.08E­04 0 0 9.95E­05
CRU kg 0 0 0 0 0 0 0 0
MFR kg 0 0 0 0 0 1.86E+02 0 0
MER kg 6.11E+00 0 0 0 0 0 0 0
EEE MJ 0 0 0 0 0 0 0 0
5 Environmental Product Declaration ­ Give Steel A/S ­ Galvanized Structural Steel
EET MJ 0 0 0 0 0 0 0 0
HWD = Hazardous waste disposed; NHWD = Non­hazardous waste disposed; RWD = Radioactive waste disposed; CRU = Components for re­use;
MFR = Materials for recycling; MER = Materials for energy recovery; EEE = Exported electrical energy; EET = Exported thermal energy
RESULTS OF THE LCA – additional impact categories according to EN 15804+A2-optional:
1 ton galvanized structural steel
Parameter Unit A1-A3 A4 A5 C1 C2 C3 C4 D
Disease
PM 3.74E­05 1.72E­07 3.76E­08 3.76E­08 1.74E­07 3.78E­06 0 3.21E­05
incidence
IR kBq U235 eq 2.66E+01 3.03E­02 3.43E­03 3.43E­03 3.06E­02 3.52E+00 0 3.85E+01
ETP­fw CTUe 2.69E+03 8.31E+01 9.4E+00 9.4E+00 8.39E+01 1.7E+03 0 4.57E+03
HTP­c CTUh 7.46E­07 1.72E­09 1.94E­10 1.94E­10 1.73E­09 3.61E­08 0 8.92E­07
HTP­nc CTUh 1.79E­05 1E­07 1.08E­08 1.08E­08 1.01E­07 1.71E­06 0 1.56E­05
SQP SQP 2.24E+03 3.9E+01 4.41E+00 4.41E+00 3.94E+01 6.98E+02 0 3.13E+03
PM = Potential incidence of disease due to PM emissions; IR = Potential Human exposure efficiency relative to U235; ETP­fw = Potential comparative
Toxic Unit for ecosystems; HTP­c = Potential comparative Toxic Unit for humans (cancerogenic); HTP­nc = Potential comparative Toxic Unit for humans
(not cancerogenic); SQP = Potential soil quality index
Disclaimer 1 – for the indicator “Potential Human exposure efficiency relative to U235”. This impact category deals mainly with the
eventual impact of low­dose ionizing radiation on human health of the nuclear fuel cycle. It does not consider effects due to possible
nuclear accidents, occupational exposure or radioactive waste disposal in underground facilities. Potential ionizing radiation from the
soil, radon and from some construction materials is also not measured by this indicator.
Disclaimer 2 – for the indicators “abiotic depletion potential for non­fossil resources”, “abiotic depletion potential for fossil resources”,
“water (user) deprivation potential, deprivation­weighted water consumption”, “potential comparative toxic unit for ecosystems”,
“potential comparative toxic unit for humans – cancerogenic”, “Potential comparative toxic unit for humans ­ not cancerogenic”,
“potential soil quality index”. The results of this environmental impact indicator shall be used with care as the uncertainties on these
results are high as there is limited experience with the indicator.
This EPD was created using a software tool.
6. LCA: Interpretation
The calculated environmental impacts primarily stem from the the production of scrap steel and ore­based steel.
production of scrap steel, which accounts for 78 % of the The structural steel product is manufactured using water,
product's weight. The production of scrap steel is the main electricity and heat at the production site in Brande, Denmark.
contributor to 6 out of 19 environmental impact categories. The These processes only have a minor effect on the overall
production of ore­based steel is the main contributor to 8 out of environmental impacts of the product. The main contributor to
19 environmental impact categories. The most dominant the environmental impacts in module A3 is heat consumption,
module is therefore module A1, since the module includes both as natural gas is used.
7. Requisite evidence
characteristic of an urban and industrial atmosphere with
7.1 Weathering Performance moderate sulfur dioxideload and a coastal atmosphere with low
The corrosion rate of zinc depends on the position of the salt load and thus corresponds to the typical corrosive load of
component and the conditions of the surrounding atmosphere steel structures, the corrosion rate is assumed to be
(corrosivity categories according to EN ISO 12944­2). For 1.3µm/year.
corrosivity category C3, which according to this standard is
8. References
Standards
EN 13479
AgBB EN 13479:2017, Welding consumables ­ General product
AgBB, Ausschuss zur gesundheitlichen Bewertung von standard for filler metals and fluxes for fusion welding of
Bauprodukten (Committee for Health­related Evaluation of metallic materials.
Building Products).
EN 13501
EN 1090 EN 13501­1:2010, Fire classification of construction products
EN 1090­2:2018, Execution of steel structures and aluminium and building elements.
structures ­ Part 2: Technical requirements for steel structures.
EN 15804
EN 10025 EN 15804:2012+A2:2019+AC:2021, Sustainability of
EN 10025­2:2019, Hot rolled products of structural steels ­ Part construction works — Environmental Product Declarations —
2: Technical delivery conditions for non­alloy structural steels. Core rules for the product category of construction products.
EN 10219 EN 16516
EN 10219­1:2006, Cold formed welded structural hollow EN 16516:2017+A1:2020, Construction products: Assessment
sections of non­alloy and fine grain steels ­ Part 1: Technical of release of dangerous substances. Determination of
delivery conditions. emissions into indoor air.
6 Environmental Product Declaration ­ Give Steel A/S ­ Galvanized Structural Steel
Eurofins Product Testing
ISO 544 https://www.eurofins.dk/product­testing/
ISO 544:2017, Welding consumables — Technical delivery
conditions for filler materials and fluxes — Type of product, EWC
dimensions, tolerances and markings. European Waste Catalogue, European Commission
ISO 12944 PCR Part A
ISO 12944­2: 2017, Paints and varnishes — Corrosion Calculation Rules for the Life Cycle Assessment and
protection of steel structures by protective paintsystems ­­ Part Requirements on the Project Report according to EN
2: Classification of environments 15804+A2:2019. Institut Bauen und Umwelt e.V. (IBU). Version
1.2. November 2021. www.ibu­epd.com
ISO 14025
ISO 14025:2011, Environmental labels and declarations — PCR Part B
Type III environmental declarations — Principles and Requirements on the EPD for www.ibu­epd.com Structural
procedures. steels. Institut Bauen und Umwelt e.V. (IBU). Version 1.1. 2017.
www.ibu­epd.com
ISO 16000-6
ISO 16000­6:2011, Indoor air ­ Part 6: Determination of volatile Software
organic compounds in indoor and test chamber air by active
sampling on Tenax TA sorbent, thermal desorption and gas GaBi Software
chromatography using MS or MSFID. Sphera Solutions GmbH. (2020). For further information see:
gabi.sphera.com/international/index
Further references
Databases
Candidate List of Substances of Very High Concern for
Authorisation GaBi Professional
Candidate List of substances of very high concern for Sphera Solutions GmbH. (2020). GaBi LCA Database
Authorisation, 2021, ECHA, echa.europa.eu Documentation. Retrieved from
gabi.sphera.com/international/support/gabi
CPR
Regulation (EU) No 305/2011 of the European Parliament and Ecoinvent 3.6
of the Council of 9 March 2011 laying down harmonised http://www.gabi­software.com/nw­eu­
conditions for the marketing of construction products and danish/databases/ecoinvent
repealing Council Directive 89/106/EEC Text with EEA
relevance. IBU 2021
Institut Bauen und Umwelt e.V.: General Instructions for the
EMICODE EPD programme of Institut Bauen und Umwelt e.V., Version
https://www.emicode.com/ 2.0, Berlin: Institut Bauen und Umwelt e.V., 2021 www.ibu­
epd.com .
7 Environmental Product Declaration ­ Give Steel A/S ­ Galvanized Structural Steel
Publisher
Institut Bauen und Umwelt e.V. +49 (0)30 3087748­ 0
Hegelplatz 1 info@ibu­epd.com
10117 Berlin www.ibu­epd.com
Germany
Programme holder
Institut Bauen und Umwelt e.V. +49 (0)30 3087748­ 0
Hegelplatz 1 info@ibu­epd.com
10117 Berlin www.ibu­epd.com
Germany
Author of the Life Cycle Assessment
COWI A/S 56 40 00 00
Parallelvej 2 cowi@cowi.com
2800 Kgs. Lyngby https://www.cowi.com/
Denmark
Owner of the Declaration
Give Steel A/S +4575731218
Sjællandsvej 14 info@givesteel.com
7330 Brande givesteel.com
Denmark
8 Environmental Product Declaration ­ Give Steel A/S ­ Galvanized Structural Steel
