ENVIRONMENTAL PRODUCT DECLARATION
as per ISO 14025 and EN 15804+A2
Owner of the Declaration
Programme holder Institut Bauen und Umwelt e.V. (IBU)
Publisher Institut Bauen und Umwelt e.V. (IBU)
Declaration number EPD-OYS-20210252-IBA1-EN
Issue date 27.11.2021
Valid to 26.11.2026
Vinyplan 6813ECO
Oy Scantarp Ab
www.ibu-epd.com | https://epd-online.com
Umwelt Produktdeklaration Name des Herstellers – Name des Produkts
1. General Information
Oy Scantarp Ab Vinyplan 6813ECO
Programme holder Owner of the declaration
IBU – Institut Bauen und Umwelt e.V. Oy Scantarp Ab
Panoramastr. 1 Lukkosalmentie 4
10178 Berlin 70420 Kuopio
Germany Finland
Declaration number Declared product / declared unit
EPD-OYS-20210252-IBA1-EN Vinyplan 6813ECO / 1 m2
This declaration is based on the product Scope:
category rules: This EPD describes Vinyplan 6813ECO, a technical
Technical Textiles, 01.2019 fabric manufactured by Oy Scantarp Ab in Kuopio,
(PCR checked and approved by the SVR) Finland.
Issue date The declared product is a fully airtight recycled
27.11.2021 polyethylene terephthalate - recycled polyvinyl chloride
(rPET-rPVC) based technical textile. The base fabric is
composed of high tenacity, low shrinkage, multifilament
Valid to
polyester yarns made from recycled PET bottles.
26.11.2026
EPD type is cradle-to-gate with modules C1-C4 and D.
The EPD is created based on the background report
including a study compiled for this product.
The owner of the declaration shall be liable for the
underlying information and evidence; the IBU shall not
be liable with respect to manufacturer information, life
cycle assessment data and evidences.
The EPD was created according to the specifications
of EN 15804+A2. In the following, the standard will be
simplified as EN 15804.
Verification
The standard EN 15804 serves as the core PCR
Independent verification of the declaration and data
according to ISO 14025:2010
Dipl. Ing. Hans Peters internally x externally
(chairman of Institut Bauen und Umwelt e.V.)
Dr. Alexander Röder Matthias Klingler
(Managing Director Institut Bauen und Umwelt e.V.)) (Independent verifier)
2. Product
2.1 Product description/Product definition rPVC) based technical textile. The base fabric is
composed of high tenacity, low shrinkage,
multifilament polyester yarns made out of recycled
PET bottles. The product is coated symmetrically on
both sides by 2 layers of coating, which include ab
adhesion layer made out of recycled PVC plastisol and
a main coating made out of recycled PVC dry blend
with several additives.
Vinyplan 6813ECO consists of best performance
REACH compliant chemicals. Due to the calendering
processing technique, the declared product is fully
airtight. The declared product weighs 620 g/m2.
For the use and application of the product, the
respective national provisions at the place of use
The declared product is a recycled polyethylene
apply, in Germany for example the building codes of
terephthalate – recycled polyvinyl chloride (rPET-
2 Environmental Product Declaration Oy Scantarp Ab – Vinyplan 6813ECO
the federal states and the corresponding national The biocide product used contains also di-
specifications. isononylphthalate CAS: 68515-48-0.
2.2 Application 2.6 Manufacture
The main area of application for 6813ECO is The manufacturing begins with the preparation of
predominantly tarps. plastisol containing internally recycled PVC plastisol,
PVC and additives. Plastisol is used as the first coating
2.3 Technical Data on the recycled base polyester fabric. Dry blend
Performance data of the product with respect to its containing internally recycled dry blend, PVC and
characteristics in accordance with the relevant additives is prepared, melted, extruded and hot
technical provision (no CE-marking). pressed into sheet, which is then calendered on the
fabric. The fabric is calendered twice, once on both
Technical specifications for Vinyplan 6813ECO sides.
Name Value Unit
Yarn About 3 % of raw material mass ends up as
Yarn count DIN EN 1049-2 6 x 7
count /cm manufacturing rejects, which are landfilled.
Linear density of yarns DIN ISO
1100 dtex
2060 The sales, marketing and production of this product
Grammage DIN EN ISO 2286-1 620 g/m2 have been certified according to the following
Tensile strength (warp/weft) DIN 2200 standard:
N/50mm
EN ISO 1421-1 2300
Tearing strength (warp/weft) DIN 220 ISO 9001
N
53363 210
Temperature resistance (cold) 2.7 Environment and health during
DIN EN 1876-1 -35 °C manufacturing
Temperature resistance (hot) +70 °C
Health protection: All production employees are
trained to work with chemicals. Safety clothes and
safety devices are provided. Regular health checks are
mandatory for all employees. The occupational
exposure limit for plasticizers is measured and values
2.4 Delivery status
are within the compulsory safety levels. The extensive
The following table includes minimum and maximum
health care program is available to all employees.
dimensions for the product supplied worldwide. Some
of the combinations for sizes may not be available.
Production waste: The waste streams from
manufacturing are sorted and most of the chemical
Min value Max Value Unit
wastes are recycled in their own production. Only the
Width 2 205 cm
PVC coated fabric rejects will be sent to landfill.
Length 6000 50000 cm
Emissions into air: Waste air generated during
For updated information on available dimensions,
production is cleaned in accordance with regulatory
please contact sales@scantarp.fi
requirements. Emissions must comply with the values
specified by the operation licenses of the site.
2.5 Base materials/Ancillary materials
The product is composed of 75-76 % of recycled PVC
Emissions into water/soil: No normal process
and 24-25 % of recycled polyester.
contamination of water or soil exists. The production
process of coated fabrics does not have any
This product/article/at least one partial article contains
production-related wastewater.
substances listed in the candidate list
(date:16.04.2021) exceeding 0.1 percentage by mass:
Noise: The measurements of noise level are
no.
performed and the results are within the compulsory
safety levels. Use of ear protection is required in the
This product/article/at least one partial article contains
production area.
other carcinogenic, mutagenic, reprotoxic
(CMR) substances in categories 1A or 1B which are
The environmental management system has been
not on the candidate list, exceeding 0.1 percentage by
certified according to the following standard:
mass: no.
ISO 14001
Biocide products were added to this construction
product or it has been treated with biocide products
2.8 Product processing/Installation
(this then concerns a treated product as defined by the
Due to Vinyplan 6813ECO being an intermediate
(EU) Ordinance on Biocide Products No. 528/2012):
product used in many different end products, no
yes.
specific description or guidance is given, as the
installation stage only applies for the specific end
According to the EU Biocidal Products Regulation
product.
(528/2012) is informed that this product contains the
biocidal product dichloro n-octyl isothiazolinone
2.9 Packaging
(DCOIT) CAS: 64359-81-5, an antifungal additive,
The product is packaged using wooden pallets,
used to help maintain appearance, physical properties
residual PVC coated fabric, paperboard roll cores and
and prolong the service life of this product as before.
plastic film and straps. The packaging is not product
packaging per se, but coverage for transport. Wooden
3 Environmental Product Declaration Oy Scantarp Ab – Vinyplan 6813ECO
pallets may be reused or refurbished. Paperboard roll
cores may be directed to cardboard recycling and 2.13 Extraordinary effects
plastic may be directed to recycling of energy recovery.
Fire
The declared product is not classified according to fire
2.10 Condition of use retardant standards.
Any harmful effects to the environment are not known.
The mechanical destruction of the declared product Water
does not alter the chemical composition. The declared product is suitable for outdoor use. The
product has good weather resistance properties. The
Regarding the emissions to soil and water, no test declared product is not biodegradable and not soluble
results are available. in water.
2.11 Environment and health during use Mechanical destruction
No specific hazards are known in normal use. The mechanical destruction of the declared product
Decomposition of the product begins at about 150 ºC does not alter the chemical composition.
by long term heating and the decomposition of
hazardous products as hydrogen chloride may occur. 2.14 Re-use phase
It is assumed that the end product, of which Vinyplan
Aerosols and solid particles may occur during heating 6813ECO is a part of, is not reused or recovered as
and high frequency welding. material.
By heating over 150 ºC vapours may irritate eyes and 2.15 Disposal
lungs, may cause headache. Skin irritation and Incineration with energy recovery is assumed to be the
eczema may occur. Use of long sleeve work wear is most plausible end-of-life scenario for Vinyplan
recommended. 6813ECO. Landfilling is considered in an alternative
scenario, in the case the product ends up disposed of.
The declared product is not biodegradable and not As a non-hazardous plastic product used in
soluble in water. construction, the waste code of Vinyplan 6813ECO
according to European Waste Catalogue is 17 02 03.
2.12 Reference service life
Due to the wide range of applications of Vinyplan 2.16 Further information
6813ECO and to the exclusion of module B, no For further information, e.g. datasheets, please contact
reference service life is declared. sales@scantarp.fi
3. LCA: Calculation rules
3.1 Declared Unit C1-C4:
The declared unit for Vinyplan 6813ECO is 1 m2 of  C1: Deconstruction of the product from
fabric. The conversion factor to mass per declared unit building.
is 0.62 kg/m2.
 C2: Transport of used product to end-of-life
treatment.
Declared unit
Name Value Unit  C4/1: Incineration with energy recovery.
Declared unit 1 m2  C4/2 (alternative scenario): Landfill disposal.
Conversion factor to 1 kg 0.62 -
D:
 Credits acquired from material and energy
recovery across the product system.
3.2 System boundary
The type of the EPD is cradle to gate with options:
including modules A1-A3, C1-C4 and D. The declared
life cycle stages and accompanying processes are 3.3 Estimates and assumptions
listed below: Flows relating to infrastructure, employee commute,
capital equipment and auxiliary electricity consumption
A1-A3: are excluded. Biogenic carbon in the product is
 A1: Production of raw materials. assumed to be completely released in landfill.
 A2: Transport of raw materials and packaging Commercial one-way transports are considered. The
product is assumed to not require waste processing or
materials to the manufacturer.
sorting activities in module C3.
 A3: Production of packaging materials, fuels,
energy and water.
3.4 Cut-off criteria
 A3: Manufacturing process and emissions Mass- and energy-based cut-off criteria are adhered
from fuels, energy and processing. to. Flows accounting for less than 1 % of the overall
 A3: Transport and treatment of wastes. input mass or energy flows in each model are excluded
from the study if appropriate LCI data or even proxy
data are not available. Additionally, the sum of
excluded flows does not exceed 5 % of the total
inflows (by mass or by energy) of each module.
4 Environmental Product Declaration Oy Scantarp Ab – Vinyplan 6813ECO
measured in 2021. Used data represent the
3.5 Background data manufacturing in Kuopio in 2020.
Secondary data from GaBi Professional and Ecoinvent
databases and literature are used in modelling. 3.8 Allocation
Wherever possible, data from GaBi are prioritised over As a principle, allocation is avoided whenever possible.
data from Ecoinvent. As principle, secondary data with When allocation is applied, it is ensured that there is
a maximum of 10 years were used in the modelling no double-counting or omissions, and all the
when available. environmental impacts are allocated to either product
or co-products.
3.6 Data quality
The best available generic datasets are used for every The consumption of fuel for heating and the use of
unit process. In addition to geographical, technical and cooling water are equally allocated between all
time representativeness assessment, other data products at the manufacturer based on their annual
quality-related viewpoints were considered when production volumes.
choosing the modelling data for upstream and
downstream processes. 3.9 Comparability
Basically, a comparison or an evaluation of EPD data
The precision of the data used is as accurate as is only possible if all the data sets to be compared
possible. Primary data are precise, but secondary were created according to EN 15804 and the building
data, such as data from the databases and literature, context, respectively the product-specific
may contain broad uncertainties. Data approximations characteristics of performance, are taken into account.
correspond to 0.8 % of raw material mass of Vinyplan
6813ECO. GaBi Professional database 2020 and Ecoinvent 3.6
database were used in the modelling. GaBi database
3.7 Period under review is used wherever possible, and Ecoinvent database is
The primary data from the manufacturer were mainly used to fill the remaining data gaps.
collected in 2020 and electricity consumption was
4. LCA: Scenarios and additional technical information
Characteristic product properties Packaging end-of-life (technical scenario for A5)
Information on biogenic Carbon Name Value Unit
Biogenic carbon content of the product and packaging Material loss 0 kg
are shown in the table below. Few additives in Packaging materials to recycling 9.8 g/m2
Vinyplan 6813ECO are biogenic. Packaging materials Packaging materials to energy
21.0 g/m2
contain paperboard and wooden materials. The mass recovery
of packaging containing biogenic carbon is 0.03 kg/m2.
Information on describing the biogenic carbon
content at factory gate End of life (C1-C4)
Name Value Unit Name Value Unit
Biogenic Carbon Content in Collected separately waste type 0.62 kg
0.004 kg C
product Collected as mixed construction
- kg
Biogenic Carbon Content in waste
0.01 kg C
accompanying packaging Reuse - kg
Recycling - kg
Energy recovery (scenario C4/1) 0.62 kg
Vinyplan 6813ECO is an intermediate product and Landfilling (scenario C4/2) 0.62 kg
therefore the transport of the product to an
intermediate user is declared as a technical scenario
Reuse, recovery and/or recycling potentials (D),
for module A4.
relevant scenario information
Name Value Unit
Transport to intermediate user (technical scenario
Materials for recycling 12.8 g/m2
for A4)
Materials for energy recovery 21.6 g/m2
Name Value Unit
Average road transport distance 360 km
Average ship transport distance 48 km
Since the use of packaging material is declared in
module A3, the end-of-life of packaging materials is
declared as the technical scenario for module A5.
Material loss is not considered in the technical
scenario for A5, since it only deals with the end-of-life
of packaging materials at intermediate user and
installation activities do not take place.
5 Environmental Product Declaration Oy Scantarp Ab – Vinyplan 6813ECO
5. LCA: Results
Note: Results for modules A4 and A5 are for the technical scenarios for the respective modules, see section 4.
Disclaimer:
EP-freshwater: This indicator has been calculated as “kg P eq” as required in the characterization model
(EUTREND model, Struijs et al., 2009b, as implemented in ReCiPe;
http://eplca.jrc.ec.europa.eu/LCDN/developerEF.xhtml).
DESCRIPTION OF THE SYSTEM BOUNDARY (X = INCLUDED IN LCA; ND = MODULE OR INDICATOR NOT
DECLARED; MNR = MODULE NOT RELEVANT)
BENEFITS AND
CONSTRUCTI LOADS
PRODUCT STAGE ON PROCESS USE STAGE END OF LIFE STAGE BEYOND THE
STAGE SYSTEM
BOUNDARIES
6 Environmental Product Declaration Oy Scantarp Ab – Vinyplan 6813ECO
lairetam
waR
ylppus tropsnarT
gnirutcafunaM
eht
morf
tropsnarT
etis
eht
ot
etag
ylbmessA esU
ecnanetniaM
riapeR
tnemecalpeR tnemhsibrufeR
ygrene
lanoitarepO esu
retaw
lanoitarepO esu
noitcurtsnoc-eD
noitilomed tropsnarT
gnissecorp
etsaW
lasopsiD -esueR -yrevoceR -gnilcyceR laitnetop
A1 A2 A3 A4 A5 B1 B2 B3 B4 B5 B6 B7 C1 C2 C3 C4 D
X X X X X ND ND MNR MNR MNR ND ND X X X X X
RESULTS OF THE LCA - ENVIRONMENTAL IMPACT according to EN 15804+A2: 1 m2 Vinyplan 6813ECO
Core Indicator Unit A1 A2 A3 A4 A5 C1 C2 C3 C4/1 C4/2 D
GWP-total [kg CO2-Eq.] 7.45E-1 3.93E-2 6.41E-1 2.00E-2 4.85E-2 3.82E-4 6.77E-3 0.00E+0 1.56E+0 4.44E-2 -4.15E-1
GWP-fossil [kg CO2-Eq.] 7.39E-1 3.92E-2 6.81E-1 1.99E-2 1.37E-2 3.97E-4 6.73E-3 0.00E+0 1.56E+0 4.49E-2 -4.28E-1
GWP-biogenic [kg CO2-Eq.] 6.10E-3 1.97E-5 -4.03E-2 -3.30E-5 3.48E-2 -1.76E-5 -1.15E-5 0.00E+0 -5.25E-4 -5.25E-4 1.39E-2
GWP-luluc [kg CO2-Eq.] 4.96E-4 8.51E-5 1.18E-4 1.59E-4 3.61E-5 3.09E-6 5.46E-5 0.00E+0 2.51E-4 3.64E-5 -3.17E-4
ODP [kg CFC11-Eq.] 4.46E-8 3.98E-18 3.99E-11 2.39E-18 9.95E-11 4.59E-20 8.11E-19 0.00E+0 1.89E-15 1.02E-16 -8.11E-10
AP [mol H+-Eq.] 3.49E-3 7.78E-4 1.40E-3 6.27E-5 1.94E-5 1.92E-6 1.89E-5 0.00E+0 3.96E-4 1.36E-4 -6.37E-4
EP-freshwater [kg P-Eq.] 1.68E-4 3.82E-8 1.12E-6 5.97E-8 3.12E-7 1.16E-9 2.05E-8 0.00E+0 3.17E-7 8.20E-6 -2.52E-6
EP-marine [kg N-Eq.] 9.35E-4 2.92E-4 3.68E-4 2.68E-5 4.27E-6 8.90E-7 8.28E-6 0.00E+0 1.29E-4 3.01E-5 -1.67E-4
EP-terrestrial [mol N-Eq.] 7.77E-3 3.20E-3 3.99E-3 3.00E-4 5.45E-5 9.86E-6 9.31E-5 0.00E+0 1.62E-3 3.30E-4 -1.78E-3
POCP [kg NMVOC-Eq.] 3.21E-3 7.88E-4 1.30E-3 5.70E-5 7.50E-4 2.50E-6 1.68E-5 0.00E+0 3.66E-4 9.81E-5 -4.79E-4
ADPE [kg Sb-Eq.] 3.65E-6 1.49E-9 2.30E-7 1.42E-9 6.85E-7 2.74E-11 4.84E-10 0.00E+0 2.72E-8 3.03E-9 -1.95E-7
ADPF [MJ] 1.13E+1 4.88E-1 1.21E+1 2.66E-1 5.05E-2 5.09E-3 8.98E-2 0.00E+0 2.31E+0 6.43E-1 -7.27E+0
[m³ world-Eq
WDP 3.49E-1 1.45E-4 1.35E-2 1.76E-4 5.87E-3 3.41E-6 6.03E-5 0.00E+0 1.25E-1 -5.03E-4 -6.81E-2
deprived]
GWP = Global warming potential; ODP = Depletion potential of the stratospheric ozone layer; AP = Acidification potential of land and water; EP =
Caption Eutrophication potential; POCP = Formation potential of tropospheric ozone photochemical oxidants; ADPE = Abiotic depletion potential for non-
fossil resources; ADPF = Abiotic depletion potential for fossil resources; WDP = Water (user) deprivation potential
RESULTS OF THE LCA - INDICATORS TO DESCRIBE RESOURCE USE according to EN 15804+A2: 1 m2
Vinyplan 6813ECO
Indicator Unit A1 A2 A3 A4 A5 C1 C2 C3 C4/1 C4/2 D
PERE [MJ] 4.46E-1 8.95E-3 4.04E-1 1.47E-2 3.25E-1 2.86E-4 5.05E-3 0.00E+0 6.91E-1 4.52E-2 -2.07E+0
PERM [MJ] 2.74E-1 0.00E+0 4.05E-1 0.00E+0 -4.57E-1 0.00E+0 0.00E+0 0.00E+0 -2.14E-1 0.00E+0 0.00E+0
PERT [MJ] 7.20E-1 8.95E-3 8.08E-1 1.47E-2 -1.32E-1 2.86E-4 5.05E-3 0.00E+0 4.77E-1 4.52E-2 -2.07E+0
PENRE [MJ] 1.13E+1 4.88E-1 1.21E+1 2.66E-1 1.91E-1 5.09E-3 8.99E-2 0.00E+0 1.41E+1 6.43E-1 -7.27E+0
PENRM [MJ] 1.22E+1 0.00E+0 1.14E-1 0.00E+0 -1.41E-1 0.00E+0 0.00E+0 0.00E+0 -1.18E+1 0.00E+0 0.00E+0
PENRT [MJ] 2.35E+1 4.88E-1 1.22E+1 2.66E-1 5.06E-2 5.09E-3 8.99E-2 0.00E+0 2.31E+0 6.43E-1 -7.27E+0
SM [kg] 6.05E-1 0.00E+0 0.00E+0 0.00E+0 0.00E+0 0.00E+0 0.00E+0 0.00E+0 0.00E+0 0.00E+0 1.28E-2
RSF [MJ] 0.00E+0 0.00E+0 0.00E+0 0.00E+0 0.00E+0 0.00E+0 0.00E+0 0.00E+0 0.00E+0 0.00E+0 0.00E+0
NRSF [MJ] 0.00E+0 0.00E+0 0.00E+0 0.00E+0 0.00E+0 0.00E+0 0.00E+0 0.00E+0 0.00E+0 0.00E+0 0.00E+0
FW [m³] 8.18E-3 1.11E-5 2.13E-3 1.70E-5 1.53E-4 3.31E-7 5.85E-6 0.00E+0 3.19E-3 7.90E-6 -2.38E-3
PERE = Use of renewable primary energy excluding renewable primary energy resources used as raw materials; PERM = Use of
renewable primary energy resources used as raw materials; PERT = Total use of renewable primary energy resources; PENRE = Use of
non-renewable primary energy excluding non-renewable primary energy resources used as raw materials; PENRM = Use of non-
Caption
renewable primary energy resources used as raw materials; PENRT = Total use of non-renewable primary energy resources; SM = Use
of secondary material; RSF = Use of renewable secondary fuels; NRSF = Use of non-renewable secondary fuels; FW = Use of net fresh
water
RESULTS OF THE LCA – WASTE CATEGORIES AND OUTPUT FLOWS according to EN 15804+A2:
1 m2 Vinyplan 6813ECO
Indicator Unit A1 A2 A3 A4 A5 C1 C2 C3 C4/1 C4/2 D
HWD [kg] 7.43E-12 6.50E-9 9.48E-9 1.22E-8 2.50E-10 2.37E-10 4.18E-9 0.00E+0 1.02E-8 2.35E-9 -2.87E-9
NHWD [kg] 1.02E-3 5.70E-5 2.50E-2 4.05E-5 1.36E-3 7.79E-7 1.38E-5 0.00E+0 7.49E-1 1.24E+0 -3.32E-3
RWD [kg] 6.06E-8 5.62E-7 1.78E-3 3.29E-7 5.69E-6 6.30E-9 1.11E-7 0.00E+0 7.47E-5 7.76E-6 -5.35E-4
CRU [kg] 0.00E+0 0.00E+0 0.00E+0 0.00E+0 0.00E+0 0.00E+0 0.00E+0 0.00E+0 0.00E+0 0.00E+0 0.00E+0
MFR [kg] 0.00E+0 0.00E+0 3.07E-3 0.00E+0 9.76E-3 0.00E+0 0.00E+0 0.00E+0 0.00E+0 0.00E+0 0.00E+0
MER [kg] 0.00E+0 0.00E+0 2.54E-4 0.00E+0 1.77E-4 0.00E+0 0.00E+0 0.00E+0 6.20E-1 0.00E+0 0.00E+0
EEE [MJ] 0.00E+0 0.00E+0 2.27E-3 0.00E+0 6.67E-2 0.00E+0 0.00E+0 0.00E+0 1.72E+0 0.00E+0 0.00E+0
EET [MJ] 0.00E+0 0.00E+0 4.06E-3 0.00E+0 1.19E-1 0.00E+0 0.00E+0 0.00E+0 3.12E+0 0.00E+0 0.00E+0
Caption HWD = Hazardous waste disposed; NHWD = Non-hazardous waste disposed; RWD = Radioactive waste disposed; CRU = Components
for re-use; MFR = Materials for recycling; MER = Materials for energy recovery; EEE = Exported electrical energy; EEE = Exported
thermal energy
RESULTS OF THE LCA – additional impact categories according to EN 15804+A2-optional:
1 m2 Vinyplan 6813ECO
Indicator Unit A1 A2 A3 A4 A5 C1 C2 C3 C4/1 C4/2 D
[Disease
PM ND ND ND ND ND ND ND ND ND ND ND
Incidence]
[kBq U235-
IRP ND ND ND ND ND ND ND ND ND ND ND
Eq.]
ETP-fw [CTUe] ND ND ND ND ND ND ND ND ND ND ND
HTP-c [CTUh] ND ND ND ND ND ND ND ND ND ND ND
HTP-nc [CTUh] ND ND ND ND ND ND ND ND ND ND ND
SQP [-] ND ND ND ND ND ND ND ND ND ND ND
PM = Potential incidence of disease due to PM emissions; IR = Potential Human exposure efficiency relative to U235; ETP-fw = Potential
Caption comparative Toxic Unit for ecosystems; HTP-c = Potential comparative Toxic Unit for humans (cancerogenic); HTP-nc = Potential
comparative Toxic Unit for humans (not cancerogenic); SQP = Potential soil quality index
Disclaimer for the indicators: “ADPF”, “ADPE”, “WDP”.The results of these environmental impact indicators shall
be used with care as the uncertainties on these results are high or as there is limited experience with the
indicators.
6. LCA: Interpretation
Dominance analysis is carried out for Vinyplan is the most significant for most impact categories,
6813ECO, illustrated in the figure below. The results of especially ODP and EP-freshwater impacts. For ADPF
module D are excluded from the analysis. stage A3 and for GWP-total and GWP-fossil stage C4
are the most relevant stages. Stage A3 is overall the
Overall, stage A1 is the most relevant life cycle stage second most relevant life cycle stage for Vinyplan
for Vinyplan 6813ECO, contributing 21.0-99.7 % to 6813ECO, contributing 0.1-45.5 % to each impact
each impact category (54.4 % on average). Stage A1 category (16.9 % on average).
7. Requisite evidence
Relevant test results and evidence on the organic compound (VOC) emissions are not declared
characteristics of Vinyplan 6813ECO product are for this product.
declared in, for example, sections 2.3, 2.6-2.7, 2.9-
2.10 and 2.13. Regarding the emissions to soil and 7.2 Leaching
water, no test results are available. Therefore, any Leaching performance tests have not been carried out
harmful effects to the environment are not known. for Vinyplan 6813ECO and thus no test results are
available on leaching and its potential environmental
7.1 VOC emissions impacts.
Vinyplan 6813ECO is an intermediate product, which is
mainly used in outdoor applications. Therefore, volatile
7 Environmental Product Declaration Oy Scantarp Ab – Vinyplan 6813ECO
8. References
Standards
DIN 53363 Other sources
DIN 53363:2003. Determining the tear resistance of
plastic film and sheeting by the trouser tear method. Candidate list
ECHA. Candidate List of substances of very high
DIN EN 1049-2 concern for Authorisation.
DIN EN 1049-2:1994. Determination of number of
threads per unit length of textile woven fabrics; Ecoinvent database
construction methods of analysis. Ecoinvent 3.6 database (cut-off).
DIN EN 1876-1 EU Biocidal Products Regulation
DIN EN 1876-1:1997. Rubber or plastics coated fabrics REGULATION (EU) No 528/2012 concerning the
- Low temperatures tests - Part 1: Bending test. making available on the market and use of biocidal
products.
DIN EN ISO 1421-1
DIN EN ISO 1421-1:2016. Rubber- or plastics-coated European Waste Catalogue
fabrics - Determination of tensile strength and European Waste Catalogue, by Commission Desicion
elongation at break. 2000/532/EC.
DIN EN ISO 2286-1 GaBi database
DIN EN ISO 2286-1:2016. Rubber- or plastics-coated GaBi Professional 2020 database.
fabrics - Determination of roll characteristics - Part 1:
Methods for determination of length, width and net IBU 2021
mass. Institut Bauen und Umwelt e.V.: General Programme
Instructions for the Preparation of EPDs at the Institut
DIN ISO 2060 Bauen und Umwelt e.V. Version 2.0, Berlin: Institut
DIN ISO 2060:1994. Textiles — Yarn from packages Bauen und Umwelt e.V., 2021. www.ibu-epd.com
— Determination of linear density (mass per unit
length) by the skein method. PCR Part A+A2
Calculation Rules for the Life Cycle Assessment and
EN 13501-1 Requirements on the Project Report according to EN
EN 13501-1, Fire classification of construction 15804+A2:2019.
products and building elements. Classification using
data from reaction to fire tests. PCR Part B
Requirements on the EPD for Technical Textiles.
EN 15804 Version 1.0, 2012.
EN 15804:2019+A2, Sustainability of construction
works — Environmental Product Declarations — Core REACH
rules for the product category of construction products. REACH Annex XVII: Restricted Substances List.
ISO 9001 Software
ISO 9001:2015, Quality management systems — GaBi ts, Version 10.5.0.78. Leinfelden-Echterdingen:
Requirements. Sphera Solutions GmbH.
ISO 14001
ISO 14001:2015, Environmental management systems
— Requirements with guidance for use.
ISO 14025
DIN EN ISO 14025:2011-10, Environmental labels and
declarations — Type III environmental declarations —
Principles and procedures.
8 Environmental Product Declaration Oy Scantarp Ab – Vinyplan 6813ECO
Publisher
Institut Bauen und Umwelt e.V. Tel +49 (0)30 3087748- 0
Panoramastr. 1 Fax +49 (0)30 3087748- 29
10178 Berlin Mail info@ibu-epd.com
Germany Web www.ibu-epd.com
Programme holder
Institut Bauen und Umwelt e.V. Tel +49 (0)30 - 3087748- 0
Panoramastr 1 Fax +49 (0)30 – 3087748 - 29
10178 Berlin Mail info@ibu-epd.com
Germany Web www.ibu-epd.com
Author of the Life Cycle
Assessment Tel +358442356995
LCA Consulting Oy Fax -
Laserkatu 6 Mail info@lca-consulting.fi
53850 Lappeenranta Web https://lca-consulting.fi/
Finland
Owner of the Declaration
Oy Scantarp Ab Tel +358 17 288 1188
Lukkosalmentie 4 Fax +358 17 465 1762
70420 Kuopio Mail sales@scantarp.fi
Finland Web https://www.scantarp.fi/
