ENVIRONMENTAL PRODUCT DECLARATION
as per ISO 14025 and EN 15804+A2
Owner of the Declaration
Programme holder Institut Bauen und Umwelt e.V. (IBU)
Publisher Institut Bauen und Umwelt e.V. (IBU)
Declaration number EPD-OYS-20210251-IBA1-EN
Issue date 27.11.2021
Valid to 26.11.2026
Vinyplan 6319
Oy Scantarp Ab
www.ibu-epd.com | https://epd-online.com
Umwelt Produktdeklaration Name des Herstellers – Name des Produkts
1. General Information
Oy Scantarp Ab Vinyplan 6319
Programme holder Owner of the declaration
IBU – Institut Bauen und Umwelt e.V. Oy Scantarp Ab
Panoramastr. 1 Lukkosalmentie 4
10178 Berlin 70420 Kuopio
Germany Finland
Declaration number Declared product / declared unit
EPD-OYS-20210251-IBA1-EN Vinyplan 6319 / 1 m2
This declaration is based on the product Scope:
category rules: This EPD describes Vinyplan 6319, a technical fabric
Technical Textiles, 01.2019 manufactured by Oy Scantarp Ab in Kuopio, Finland.
(PCR checked and approved by the SVR)
The declared product is a fully airtight polyethylene
Issue date terephthalate - polyvinyl chloride (PET-PVC) based
27.11.2021 technical textile. The base fabric is composed of high
tenacity, low shrinkage, multifilament polyester yarns.
Valid to
26.11.2026 EPD type is cradle-to-gate with modules C1-C4 and D.
The EPD is created based on the background report
including a study compiled for this product.
The owner of the declaration shall be liable for the
underlying information and evidence; the IBU shall not
be liable with respect to manufacturer information, life
cycle assessment data and evidences.
The EPD was created according to the specifications
of EN 15804+A2. In the following, the standard will be
simplified as EN 15804.
Verification
The standard EN 15804 serves as the core PCR
Independent verification of the declaration and data
according to ISO 14025:2010
Dipl. Ing. Hans Peters internally x externally
(chairman of Institut Bauen und Umwelt e.V.)
Dr. Alexander Röder Matthias Klingler
(Managing Director Institut Bauen und Umwelt e.V.)) (Independent verifier)
2. Product
2.1 Product description/Product definition shrinkage, multifilament polyester yarns. The product
is coated symmetrically on both sides by 2 layers of
coating, which include adhesion layer and main
coating made out of PVC with several additives.
Vinyplan 6319 is made with best performance REACH
compliant chemicals. Due to the calendering
processing technique, the declared product is fully
airtight. The declared product weighs 700 g/m2.
For the use and application of the product, the
respective national provisions at the place of use
apply, in Germany for example the building codes of
the federal states and the corresponding national
specifications.
The declared product is a polyethylene terephthalate - 2.2 Application
polyvinyl chloride (PET-PVC) based technical textile. The range of applications for 6319 is fabric material
The base fabric is composed of high tenacity, low
2 Environmental Product Declaration Oy Scantarp Ab – Vinyplan 6319
mainly for storage curtains, partition curtains, 2.6 Manufacture
temporary silo and protective covers. The manufacturing begins with the preparation of
plastisol containing PVC, plasticizer and additives.
2.3 Technical Data Plastisol is used as the first coating on the base
Performance data of the product with respect to its polyester fabric. Dry blend containing PVC, plasticizer
characteristics in accordance with the relevant and additives is prepared, melted, extruded and hot
technical provision (no CE-marking). pressed into sheet, which is then calendered on the
fabric. The fabric is calendered twice, once on both
Technical specifications for Vinyplan 6319 sides.
Name Value Unit
Yarn About 12 % of raw material mass ends up as
Yarn count DIN EN 1049-2 8 x 9
count /cm manufacturing rejects. PVC and plasticizer rejects are
Linear density of yarns DIN ISO used in other products (10 %), while fabric rejects are
1100 dtex
2060 landfilled (2 %).
Grammage DIN EN ISO 2286-1 700 g/m2
Tensile strength (warp/weft) DIN 3000 The sales, marketing and production of this product
N/50mm
EN ISO 1421-1 3000 have been certified according to the following
Tearing strength (warp/weft) DIN 400 standard:
N
53363 400
Temperature resistance (cold) ISO 9001
-35 °C
DIN EN 1876-1
Temperature resistance (hot) +70 °C 2.7 Environment and health during
manufacturing
Health protection: All production employees are
trained to work with chemicals. Safety clothes and
safety devices are provided. Regular health checks are
2.4 Delivery status
mandatory for all employees. The occupational
The following table includes minimum and maximum
exposure limit for plasticizers is measured and values
dimensions for the product supplied worldwide. Some
are within the compulsory safety levels. The extensive
of the combinations for sizes may not be available.
health care program is available to all employees.
Min value Max Value Unit
Production waste: The waste streams from
Width 2 205 cm
manufacturing are sorted and most of the chemical
Length 6000 50000 cm
wastes are recycled in their own production. Only the
PVC coated fabric rejects will be sent to landfill.
For updated information on available dimensions,
please contact sales@scantarp.fi
Emissions into air: Waste air generated during
production is cleaned in accordance with regulatory
2.5 Base materials/Ancillary materials
requirements. Emissions must comply with the values
The product is composed of 72-73 % of PVC and 27-
specified by the operation licenses of the site.
28 % of polyester.
Emissions into water/soil: No normal process
This product/article/at least one partial article contains
contamination of water or soil exists. The production
substances listed in the candidate list
process of coated fabrics does not have any
(date:16.04.2021) exceeding 0.1 percentage by mass:
production-related wastewater.
no.
Noise: The measurements of noise level are
This product/article/at least one partial article contains
performed and the results are within the compulsory
other carcinogenic, mutagenic, reprotoxic (CMR)
safety levels. Use of ear protection is required in the
substances in categories 1A or 1B which are not on
production area.
the candidate list, exceeding 0.1 percentage by mass:
no.
The environmental management system has been
certified according to the following standard:
Biocide products were added to this construction
product or it has been treated with biocide products
ISO 14001
(this then concerns a treated product as defined by the
(EU) Ordinance on Biocide Products No. 528/2012):
2.8 Product processing/Installation
yes.
Due to Vinyplan 6319 being an intermediate product
used in many different end products, no specific
According to the EU Biocidal Products Regulation
description or guidance is given, as the installation
(528/2012) is informed that this product contains the
stage only applies for the specific end product.
biocidal product dichloro n-octyl isothiazolinone
(DCOIT) CAS: 64359-81-5, an antifungal additive,
2.9 Packaging
used to help maintain appearance, physical properties
The product is packaged using wooden pallets,
and prolong the service life of this product as before.
residual PVC coated fabric, paperboard roll cores and
The biocide product used contains also di-
plastic film and straps. The packaging is not product
isononylphthalate CAS: 68515-48-0.
packaging per se, but coverage for transport. Wooden
pallets may be reused or refurbished. Paperboard roll
cores may be directed to cardboard recycling and
plastic may be directed to recycling of energy recovery.
3 Environmental Product Declaration Oy Scantarp Ab – Vinyplan 6319
2.13 Extraordinary effects
2.10 Condition of use
Any harmful effects to the environment are not known. Fire
The mechanical destruction of the declared product The declared product is not classified according to fire
does not alter the chemical composition. retardant standards.
Regarding the emissions to soil and water, no test Water
results are available. The declared product is suitable for outdoor use. The
product has good weather resistance properties. The
2.11 Environment and health during use declared product is not biodegradable and not soluble
No specific hazards are known in normal use. in water.
Decomposition of the product begins at about 150 ºC
by long term heating and the decomposition of Mechanical destruction
hazardous products as hydrogen chloride may occur. The mechanical destruction of the declared product
does not alter the chemical composition.
Aerosols and solid particles may occur during heating
and high frequency welding. 2.14 Re-use phase
It is assumed that the end product, of which Vinyplan
By heating over 150 ºC vapours may irritate eyes and 6319 is a part of, is not reused or recovered as
lungs, may cause headache. Skin irritation and material.
eczema may occur. Use of long sleeve work wear is
recommended. 2.15 Disposal
Incineration with energy recovery is assumed to be the
The declared product is not biodegradable and not most plausible end-of-life scenario for Vinyplan 6319.
soluble in water. Landfilling is considered in an alternative scenario, in
the case the product ends up disposed of. As a non-
2.12 Reference service life hazardous plastic product used in construction, the
Due to the wide range of applications of Vinyplan 6319 waste code of Vinyplan 6319 according to European
and to the exclusion of module B, no reference service Waste Catalogue is 17 02 03.
life is declared.
2.16 Further information
For further information, e.g. datasheets, please contact
sales@scantarp.fi
3. LCA: Calculation rules
3.1 Declared Unit C1-C4:
The declared unit for Vinyplan 6319 is 1 m2 of fabric.  C1: Deconstruction of the product from
The conversion factor to mass per declared unit is 0.7 building.
kg/m2.
 C2: Transport of used product to end-of-life
treatment.
Declared unit
Name Value Unit  C4/1: Incineration with energy recovery.
Declared unit 1 m2  C4/2 (alternative scenario): Landfill disposal.
Conversion factor to 1 kg 0.7 -
D:
 Credits acquired from material and energy
recovery across the product system.
3.2 System boundary
The type of the EPD is cradle to gate with options:
including modules A1-A3, C1-C4 and D. The declared 3.3 Estimates and assumptions
life cycle stages and accompanying processes are Flows relating to infrastructure, employee commute,
listed below: capital equipment and auxiliary electricity consumption
are excluded. Biogenic carbon in the product is
A1-A3: assumed to be completely released in landfill.
 A1: Production of raw materials. Commercial one-way transports are considered. The
 A2: Transport of raw materials and packaging product is assumed to not require waste processing or
sorting activities in module C3.
materials to the manufacturer.
 A3: Production of packaging materials, fuels,
3.4 Cut-off criteria
energy and water.
Mass- and energy-based cut-off criteria are adhered
 A3: Manufacturing process and emissions to. Flows accounting for less than 1 % of the overall
from fuels, energy and processing. input mass or energy flows in each model are excluded
 A3: Transport and treatment of wastes. from the study if appropriate LCI data or even proxy
data are not available. Additionally, the sum of
excluded flows does not exceed 5 % of the total
inflows (by mass or by energy) of each module.
4 Environmental Product Declaration Oy Scantarp Ab – Vinyplan 6319
3.5 Background data measured in 2021. Used data represent the
Secondary data from GaBi Professional and Ecoinvent manufacturing in Kuopio production plant in Finland.
databases and literature are used in modelling.
Wherever possible, data from GaBi are prioritised over 3.8 Allocation
data from Ecoinvent. As a principle, secondary data As a principle, allocation is avoided whenever possible.
with a maximum of 10 years were used in the When allocation is applied, it is ensured that there is
modelling when available. no double counting or omissions, and all the
environmental impacts are allocated to either product
3.6 Data quality or co-products.
The best available generic datasets are used for every
unit process. In addition to geographical, technical and The consumption of fuel for heating and the use of
time representativeness assessment, other data cooling water are equally allocated between all
quality-related viewpoints were considered when products at the manufacturer based on their annual
choosing the modelling data for upstream and production volumes.
downstream processes.
3.9 Comparability
The precision of the data used is as accurate as Basically, a comparison or an evaluation of EPD data
possible. Primary data are precise, but secondary is only possible if all the data sets to be compared
data, such as data from the databases and literature, were created according to EN 15804 and the building
may contain broad uncertainties. Data approximations context, respectively the product-specific
correspond to 2.9 % of raw material mass of Vinyplan characteristics of performance, are taken into account.
6319.
GaBi Professional database 2020 and Ecoinvent 3.6
3.7 Period under review database were used in the modelling. GaBi database
The primary data from the manufacturer were mainly is used wherever possible, and Ecoinvent database is
collected in 2020 and electricity consumption was used to fill the remaining data gaps.
4. LCA: Scenarios and additional technical information
Characteristic product properties
Information on biogenic Carbon
Biogenic carbon content of the product and packaging
are shown in the table below. Few additives in End of life (C1-C4)
Vinyplan 6319 are biogenic. Packaging materials Name Value Unit
contain paperboard and wooden materials. The mass Collected separately 0.7 kg
of packaging containing biogenic carbon is 0.03 kg/m2. Collected as mixed construction
- kg
waste
Information on describing the biogenic carbon Reuse - kg
content at factory gate Recycling - kg
Name Value Unit Energy recovery (scenario C4/1) 0.7 kg
Biogenic Carbon Content in 0.009 kg C Landfilling (scenario C4/2) 0.7 kg
product
Biogenic Carbon Content in 0.01 kg C Reuse, recovery and/or recycling potentials (D),
accompanying packaging relevant scenario information
Name Value Unit
Materials for recycling 13.0 g/m2
Vinyplan 6319 is an intermediate product and therefore Materials for energy recovery 29.7 g/m2
the transport of the product to an intermediate user is
declared as a technical scenario for module A4.
Transport to intermediate user (technical scenario
for A4)
Name Value Unit
Average road transport distance 432 km
Average ship transport distance 145 km
Since the use of packaging material is declared in
module A3, the end-of-life of packaging materials is
declared as the technical scenario for module A5.
Material loss is not considered in the technical
scenario for A5, since it only deals with the end-of-life
of packaging materials at intermediate user and
installation activities do not take place.
Packaging end-of-life (technical scenario for A5)
Name Value Unit
Material loss 0 kg
Packaging materials to recycling 8.3 g/m2
Packaging materials to energy
26.5 g/m2
recovery
5 Environmental Product Declaration Oy Scantarp Ab – Vinyplan 6319
5. LCA: Results
Note: Results for modules A4 and A5 are for the technical scenarios for the respective modules, see section 4.
Disclaimer:
EP-freshwater: This indicator has been calculated as “kg P eq” as required in the characterization model
(EUTREND model, Struijs et al., 2009b, as implemented in ReCiPe;
http://eplca.jrc.ec.europa.eu/LCDN/developerEF.xhtml).
DESCRIPTION OF THE SYSTEM BOUNDARY (X = INCLUDED IN LCA; ND = MODULE OR INDICATOR NOT
DECLARED; MNR = MODULE NOT RELEVANT)
BENEFITS AND
CONSTRUCTI LOADS
PRODUCT STAGE ON PROCESS USE STAGE END OF LIFE STAGE BEYOND THE
STAGE SYSTEM
BOUNDARIES
6 Environmental Product Declaration Oy Scantarp Ab – Vinyplan 6319
lairetam
waR
ylppus tropsnarT
gnirutcafunaM
eht
morf
tropsnarT
etis
eht
ot
etag
ylbmessA esU
ecnanetniaM
riapeR
tnemecalpeR tnemhsibrufeR
ygrene
lanoitarepO esu
retaw
lanoitarepO esu
noitcurtsnoc-eD
noitilomed tropsnarT
gnissecorp
etsaW
lasopsiD -esueR -yrevoceR -gnilcyceR laitnetop
A1 A2 A3 A4 A5 B1 B2 B3 B4 B5 B6 B7 C1 C2 C3 C4 D
X X X X X ND ND MNR MNR MNR ND ND X X X X X
RESULTS OF THE LCA - ENVIRONMENTAL IMPACT according to EN 15804+A2: 1 m2 Vinyplan 6319
Core Indicator Unit A1 A2 A3 A4 A5 C1 C2 C3 C4/1 C4/2 D
GWP-total [kg CO2-Eq.] 2.27E+0 9.66E-2 7.60E-1 2.79E-2 5.73E-2 4.31E-4 7.64E-3 0.00E+0 1.78E+0 6.84E-2 -4.75E-1
GWP-fossil [kg CO2-Eq.] 2.23E+0 9.62E-2 8.04E-1 2.77E-2 1.28E-2 4.48E-4 7.59E-3 0.00E+0 1.76E+0 5.07E-2 -4.88E-1
GWP-biogenic [kg CO2-Eq.] -1.75E-2 -2.86E-5 -4.46E-2 -4.38E-5 4.45E-2 -1.98E-5 -1.30E-5 0.00E+0 1.77E-2 1.77E-2 1.32E-2
GWP-luluc [kg CO2-Eq.] 5.68E-2 4.20E-4 1.43E-4 2.16E-4 3.16E-5 3.49E-6 6.17E-5 0.00E+0 2.73E-4 4.11E-5 -3.58E-4
ODP [kg CFC11-Eq.] 1.37E-8 2.51E-17 6.44E-11 3.31E-18 8.44E-11 5.18E-20 9.15E-19 0.00E+0 2.06E-15 1.15E-16 -7.82E-10
AP [mol H+-Eq.] 6.17E-3 1.29E-3 1.68E-3 1.04E-4 1.91E-5 2.16E-6 2.13E-5 0.00E+0 4.36E-4 1.53E-4 -7.19E-4
EP-freshwater [kg P-Eq.] 1.01E-4 1.69E-7 1.14E-6 8.12E-8 2.65E-7 1.31E-9 2.31E-8 0.00E+0 3.45E-7 9.26E-6 -2.53E-6
EP-marine [kg N-Eq.] 1.37E-3 4.88E-4 4.34E-4 4.36E-5 4.50E-6 1.00E-6 9.35E-6 0.00E+0 1.42E-4 3.40E-5 -1.89E-4
EP-terrestrial [mol N-Eq.] 1.35E-2 5.36E-3 4.71E-3 4.86E-4 5.85E-5 1.11E-5 1.05E-4 0.00E+0 1.79E-3 3.73E-4 -2.01E-3
POCP [kg NMVOC-Eq.] 5.28E-3 1.29E-3 1.60E-3 9.69E-5 6.38E-4 2.82E-6 1.89E-5 0.00E+0 4.02E-4 1.11E-4 -5.40E-4
ADPE [kg Sb-Eq.] 1.45E-5 5.03E-9 3.46E-7 1.94E-9 5.81E-7 3.09E-11 5.46E-10 0.00E+0 2.96E-8 3.42E-9 -2.00E-7
ADPF [MJ] 5.44E+1 1.23E+0 1.47E+1 3.69E-1 4.83E-2 5.74E-3 1.01E-1 0.00E+0 2.52E+0 7.26E-1 -8.28E+0
[m³ world-Eq
WDP 1.50E+0 6.87E-4 1.50E-2 2.40E-4 6.62E-3 3.86E-6 6.81E-5 0.00E+0 1.41E-1 -5.68E-4 -7.34E-2
deprived]
GWP = Global warming potential; ODP = Depletion potential of the stratospheric ozone layer; AP = Acidification potential of land and water; EP =
Caption Eutrophication potential; POCP = Formation potential of tropospheric ozone photochemical oxidants; ADPE = Abiotic depletion potential for non-
fossil resources; ADPF = Abiotic depletion potential for fossil resources; WDP = Water (user) deprivation potential
RESULTS OF THE LCA - INDICATORS TO DESCRIBE RESOURCE USE according to EN 15804+A2: 1 m2
Vinyplan 6319
Indicator Unit A1 A2 A3 A4 A5 C1 C2 C3 C4/1 C4/2 D
PERE [MJ] 3.37E+0 4.56E-2 5.64E-1 2.00E-2 4.28E-1 3.23E-4 5.70E-3 0.00E+0 8.79E-1 5.10E-2 -2.27E+0
PERM [MJ] 5.05E-1 0.00E+0 4.40E-1 0.00E+0 -5.39E-1 0.00E+0 0.00E+0 0.00E+0 -3.59E-1 0.00E+0 0.00E+0
PERT [MJ] 3.87E+0 4.56E-2 1.00E+0 2.00E-2 -1.11E-1 3.23E-4 5.70E-3 0.00E+0 5.20E-1 5.10E-2 -2.27E+0
PENRE [MJ] 3.96E+1 1.23E+0 1.48E+1 3.70E-1 4.81E-1 5.75E-3 1.02E-1 0.00E+0 1.59E+1 7.26E-1 -8.28E+0
PENRM [MJ] 1.49E+1 0.00E+0 4.35E-2 0.00E+0 -4.33E-1 0.00E+0 0.00E+0 0.00E+0 -1.33E+1 0.00E+0 0.00E+0
PENRT [MJ] 5.45E+1 1.23E+0 1.48E+1 3.70E-1 4.83E-2 5.75E-3 1.02E-1 0.00E+0 2.52E+0 7.26E-1 -8.28E+0
SM [kg] 9.38E-3 0.00E+0 0.00E+0 0.00E+0 0.00E+0 0.00E+0 0.00E+0 0.00E+0 0.00E+0 0.00E+0 7.67E-2
RSF [MJ] 0.00E+0 0.00E+0 0.00E+0 0.00E+0 0.00E+0 0.00E+0 0.00E+0 0.00E+0 0.00E+0 0.00E+0 0.00E+0
NRSF [MJ] 0.00E+0 0.00E+0 0.00E+0 0.00E+0 0.00E+0 0.00E+0 0.00E+0 0.00E+0 0.00E+0 0.00E+0 0.00E+0
FW [m³] 3.60E-2 5.40E-5 2.75E-3 2.32E-5 1.69E-4 3.74E-7 6.60E-6 0.00E+0 3.60E-3 8.91E-6 -2.62E-3
PERE = Use of renewable primary energy excluding renewable primary energy resources used as raw materials; PERM = Use of
renewable primary energy resources used as raw materials; PERT = Total use of renewable primary energy resources; PENRE = Use of
non-renewable primary energy excluding non-renewable primary energy resources used as raw materials; PENRM = Use of non-
Caption
renewable primary energy resources used as raw materials; PENRT = Total use of non-renewable primary energy resources; SM = Use
of secondary material; RSF = Use of renewable secondary fuels; NRSF = Use of non-renewable secondary fuels; FW = Use of net fresh
water
RESULTS OF THE LCA – WASTE CATEGORIES AND OUTPUT FLOWS according to EN 15804+A2:
1 m2 Vinyplan 6319
Indicator Unit A1 A2 A3 A4 A5 C1 C2 C3 C4/1 C4/2 D
HWD [kg] 2.16E-4 3.21E-8 1.10E-8 1.65E-8 2.78E-10 2.67E-10 4.72E-9 0.00E+0 1.11E-8 2.65E-9 -3.27E-9
NHWD [kg] 2.18E-2 1.68E-4 2.15E-2 5.58E-5 1.56E-3 8.80E-7 1.55E-5 0.00E+0 8.13E-1 1.40E+0 -3.79E-3
RWD [kg] 7.07E-4 3.24E-6 2.37E-3 4.56E-7 5.05E-6 7.11E-9 1.26E-7 0.00E+0 8.17E-5 8.76E-6 -6.11E-4
CRU [kg] 0.00E+0 0.00E+0 5.23E-2 0.00E+0 0.00E+0 0.00E+0 0.00E+0 0.00E+0 0.00E+0 0.00E+0 0.00E+0
MFR [kg] 0.00E+0 0.00E+0 1.62E-2 0.00E+0 8.28E-3 0.00E+0 0.00E+0 0.00E+0 0.00E+0 0.00E+0 0.00E+0
MER [kg] 0.00E+0 0.00E+0 3.20E-3 0.00E+0 2.65E-2 0.00E+0 0.00E+0 0.00E+0 7.00E-1 0.00E+0 0.00E+0
EEE [MJ] 0.00E+0 0.00E+0 6.22E-3 0.00E+0 7.94E-2 0.00E+0 0.00E+0 0.00E+0 1.96E+0 0.00E+0 0.00E+0
EET [MJ] 0.00E+0 0.00E+0 1.12E-2 0.00E+0 2.15E-1 0.00E+0 0.00E+0 0.00E+0 3.55E+0 0.00E+0 0.00E+0
Caption HWD = Hazardous waste disposed; NHWD = Non-hazardous waste disposed; RWD = Radioactive waste disposed; CRU = Components
for re-use; MFR = Materials for recycling; MER = Materials for energy recovery; EEE = Exported electrical energy; EEE = Exported
thermal energy
RESULTS OF THE LCA – additional impact categories according to EN 15804+A2-optional:
1 m2 Vinyplan 6319
Indicator Unit A1 A2 A3 A4 A5 C1 C2 C3 C4/1 C4/2 D
[Disease
PM ND ND ND ND ND ND ND ND ND ND ND
Incidence]
[kBq U235-
IRP ND ND ND ND ND ND ND ND ND ND ND
Eq.]
ETP-fw [CTUe] ND ND ND ND ND ND ND ND ND ND ND
HTP-c [CTUh] ND ND ND ND ND ND ND ND ND ND ND
HTP-nc [CTUh] ND ND ND ND ND ND ND ND ND ND ND
SQP [-] ND ND ND ND ND ND ND ND ND ND ND
PM = Potential incidence of disease due to PM emissions; IR = Potential Human exposure efficiency relative to U235; ETP-fw = Potential
Caption comparative Toxic Unit for ecosystems; HTP-c = Potential comparative Toxic Unit for humans (cancerogenic); HTP-nc = Potential
comparative Toxic Unit for humans (not cancerogenic); SQP = Potential soil quality index
Disclaimer for the indicators: “ADPF”, “ADPE”, “WDP”.The results of these environmental impact indicators shall
be used with care as the uncertainties on these results are high or as there is limited experience with the
indicators.
6. LCA: Interpretation
Dominance analysis is carried out for Vinyplan 6319, impact category (70.8 % on average). Stage A1 is the
illustrated in the figure below. The results of module D most significant for every impact category, especially
are excluded from the analysis. GWP-luluc, ODP, EP-freshwater, ADPE and WDP
impacts. Stage A3 is the second most relevant life
Overall, stage A1 is the most relevant life cycle stage cycle stage for Vinyplan 6319, contributing 0.2-20.1 %
for Vinyplan 6319, contributing 45.2-98.9 % to each to each impact category (10.9 % on average).
7. Requisite evidence
Relevant test results and evidence on the organic compound (VOC) emissions are not declared
characteristics of Vinyplan 6319 product are declared for this product.
in, for example, sections 2.3, 2.6-2.7, 2.9-2.10 and
2.13. Regarding the emissions to soil and water, no
test results are available. Therefore, any harmful 7.2 Leaching
effects to the environment are not known. Leaching performance tests have not been carried out
for Vinyplan 6319 and thus no test results are available
7.1 VOC emissions on leaching and its potential environmental impacts.
Vinyplan 6319 is an intermediate product, which is
mainly used in outdoor applications. Therefore, volatile
7 Environmental Product Declaration Oy Scantarp Ab – Vinyplan 6319
8. References
Standards DIN EN ISO 14025:2011-10, Environmental labels and
declarations — Type III environmental declarations —
DIN 53363 Principles and procedures.
DIN 53363:2003. Determining the tear resistance of
plastic film and sheeting by the trouser tear method.
Other sources
DIN EN 1049-2
DIN EN 1049-2:1994. Determination of number of Candidate list
threads per unit length of textile woven fabrics; ECHA. Candidate List of substances of very high
construction methods of analysis. concern for Authorisation.
DIN EN 1876-1 Ecoinvent database
DIN EN 1876-1:1997. Rubber or plastics coated fabrics Ecoinvent 3.6 database (cut-off).
- Low temperatures tests - Part 1: Bending test.
EU Biocidal Products Regulation
DIN EN ISO 1421-1 REGULATION (EU) No 528/2012 concerning the
DIN EN ISO 1421-1:2016. Rubber- or plastics-coated making available on the market and use of biocidal
fabrics - Determination of tensile strength and products.
elongation at break.
European Waste Catalogue
DIN EN ISO 2286-1 European Waste Catalogue, by Commission Desicion
DIN EN ISO 2286-1:2016. Rubber- or plastics-coated 2000/532/EC.
fabrics - Determination of roll characteristics - Part 1:
Methods for determination of length, width and net GaBi database
mass. GaBi Professional 2020 database.
DIN ISO 2060 IBU 2021
DIN ISO 2060:1994. Textiles — Yarn from packages Institut Bauen und Umwelt e.V.: General Programme
— Determination of linear density (mass per unit Instructions for the Preparation of EPDs at the Institut
length) by the skein method. Bauen und Umwelt e.V. Version 2.0, Berlin: Institut
Bauen und Umwelt e.V., 2021. www.ibu-epd.com
EN 13501-1
EN 13501-1, Fire classification of construction PCR Part A+A2
products and building elements. Classification using Calculation Rules for the Life Cycle Assessment and
data from reaction to fire tests. Requirements on the Project Report according to EN
15804+A2:2019.
EN 15804
EN 15804:2019+A2, Sustainability of construction PCR Part B
works — Environmental Product Declarations — Core Requirements on the EPD for Technical Textiles.
rules for the product category of construction products. Version 1.0, 2012.
ISO 9001 REACH
ISO 9001:2015, Quality management systems — REACH Annex XVII: Restricted Substances List.
Requirements.
Software
ISO 14001 GaBi ts, Version 10.5.0.78. Leinfelden-Echterdingen:
ISO 14001:2015, Environmental management systems Sphera Solutions GmbH.
— Requirements with guidance for use.
ISO 14025
8 Environmental Product Declaration Oy Scantarp Ab – Vinyplan 6319
Publisher
Institut Bauen und Umwelt e.V. Tel +49 (0)30 3087748- 0
Panoramastr. 1 Fax +49 (0)30 3087748- 29
10178 Berlin Mail info@ibu-epd.com
Germany Web www.ibu-epd.com
Programme holder
Institut Bauen und Umwelt e.V. Tel +49 (0)30 - 3087748- 0
Panoramastr 1 Fax +49 (0)30 – 3087748 - 29
10178 Berlin Mail info@ibu-epd.com
Germany Web www.ibu-epd.com
Author of the Life Cycle
Assessment Tel +358 44 235 6995
LCA Consulting Oy Fax -
Laserkatu 6 Mail info@lca-consulting.fi
53850 Lappeenranta Web https://lca-consulting.fi/
Finland
Owner of the Declaration
Oy Scantarp Ab Tel +358 17 288 1188
Lukkosalmentie 4 Fax +358 17 465 1762
70420 Kuopio Mail sales@scantarp.fi
Finland Web https://www.scantarp.fi/
