ENVIRONMENTAL PRODUCT DECLARATION
as per ISO 14025 and EN 15804+A2
Owner of the Declaration MKT Metall-Kunststoff-Technik GmbH & Co. KG
Publisher Institut Bauen und Umwelt e.V. (IBU)
Programme holder Institut Bauen und Umwelt e.V. (IBU)
Declaration number EPD-MKT-20240313-CAA1-EN
Issue date 17.01.2023
Valid to 16.01.2028
VMU plus
MKT Metall-Kunststoff-Technik GmbH&Co.
KG
www.ibu-epd.com | https://epd-online.com
General Information
MKT Metall-Kunststoff-Technik GmbH&Co. VMU plus
KG
Programme holder Owner of the declaration
IBU – Institut Bauen und Umwelt e.V. MKT Metall-Kunststoff-Technik GmbH & Co. KG
Hegelplatz 1 Auf dem Immel 2
10117 Berlin 67685 Weilerbach
Germany Germany
Declaration number Declared product / declared unit
EPD-MKT-20240313-CAA1-EN The declared product is the two-component reaction resin mortar "VMU
plus", manufacturated by MKT Metall-Kunststoff-Technik GmbH&Co. KG.
The declared unit is based on 1 kg reaction resin product in the ratio at
which the two components must be mixed before use. The packaging is
also included in the calculation, since the product is sold by MKT Metall-
Kunststoff-Technik GmbH&Co. KG with its packaging. The declared unit is
indicated in [kg].
This declaration is based on the product category rules: Scope:
Reaction resin products, 01.08.2021 This document covers the two-component reaction resin mortar "VMU
(PCR checked and approved by the SVR) plus". To prepare the life cycle assessment [LCA], specific data were
collected from the MKT Metall-Kunststoff-Technik GmbH&Co. KG
manufacturing facility in Germany. The assessment is based on data from
Issue date 2020 which correspond to the yearly average. The procedure by which the
data are allocated to the declared unit is described in the "Allocation"
17.01.2023
section.
The owner of the declaration shall be liable for the underlying information
and evidence; the IBU shall not be liable with respect to manufacturer
Valid to
information, life cycle assessment data and evidences.
16.01.2028
The EPD was created according to the specifications of EN 15804+A2. In
the following, the standard will be simplified as EN 15804.
Verification
The standard EN 15804 serves as the core PCR
Independent verification of the declaration and data according to ISO
14025:2011
internally X externally
Dipl.-Ing. Hans Peters
(Chairman of Institut Bauen und Umwelt e.V.)
Florian Pronold Angela Schindler,
(Managing Director Institut Bauen und Umwelt e.V.) (Independent verifier)
1 Environmental Product Declaration - MKT Metall-Kunststoff-Technik GmbH&Co. KG - VMU plus
Product
+5°C 25 min.
Product description/Product definition +10°C 15 min.
The declared product VMU plus is a two-component reaction +20°C 6 min.
resin mortar based on vinyl ester resin that is delivered in a +30°C 4 min.
two-component plastic cartridge. The high-performance product +35°C 2 min.
is applied through a static mixer using a manual, battery- +40°C 1.5 min.
operated or pneumatic gun. It was specially developed for use
in securing threaded rods, rebar or internally threaded sleeves Curing time in dry substrate:
in solid brick, concrete, autoclaved aerated concrete and -10°C 1440 min.
lightweight concrete. Due to its excellent mechanical strength, it -5°C 840 min.
can also be used in perforated brick by using a special 0°C 420 min.
perforated sleeve. VMU plus mortar has a wide range of +5°C 120 min.
possible applications at installation tempeartures as low as -10 +10°C 80 min.
°C and operating temperatures of up to 120 °C, and offers high +20°C 45 min.
chemical resistance in extreme environments like swimming +30°C 25 min.
pools (chlorine) or near the sea (salt). With its broad range of +35°C 20 min.
national and international approvals and certifications, it can be +40°C 15 min.
used in almost any application.
Marketing of the product in the EU/EFTA (except for
Switzerland) is governed by Regulation (EU) No. 305/2011 For more information, please refer to the relevant technical data
(CPR). The product requires a Declaration of Performance sheet.
subject to ETA-11/0415, ETA-13/0909, ETA-11/0514 and CE
marking. Product performance values in accordance with the Declaration
of Performance with regard to its principal charateristics
Application
according to ETA-11/0415, ETA-13/0909 and ETA-11/0514.
The declared product VMU plus is used to reliably secure
threaded rods, internally threaded sleeves and post-installed Base materials/Ancillary materials
rebar connections in dry and moist concrete or masonry. The The declared product VMU plus is delivered as a two-
VMU plus product can also be used for water-filled boreholes. component plastic cartridge and consists of a resin component
The declared product VMU plus has very good mechanical and and a curing agent component in a 10:1 volume ratio. The
thermal properties as well as very high chemical resistance. It mixing ratio between the resin component and the curing agent
can be used in aggressive environments. The declared product component is set automatically as the product is pushed out of
VMU plus emits only a slight odour. the cartridge. Curing begins immediately after the components
are mixed.
Sample applications
Suitable for securing façades, canopies, wooden structures,
metal structures, metal profiles, supports, beams, panels, 1) "This product/article/at least one partial article contains
railings, gratings, plumbing fixtures, pipes, cable trays, post- substances in the ECHA candidate list of substances of very
installed rebar connections (for renovations or reinforcement), high concern (SVHC) (10 June 2022) above a concentration of
etc. 0.1% by mass: no."
Technical Data
The following construction data are relevant for the declared
product VMU plus as delivered: 2) "This product/article/at least one partial article contains other
Construction data CMR substances in categories 1A or 1B which are not on the
candidate list, exceeding 0.1 percentage by mass: no"
Name Value Unit
Density acc. to DIN 51757 for mixing the two
1.6 g/ml
components
Compressive strength acc. to DIN EN 196 Part 1 100.6N/mm² 3)"Biocide products were added to this construction product or
Flexural strength acc. to DIN EN 196 Part 1 14.7 N/mm² it has been treated with biocide products (this then concerns a
treated product as defined by the (EU) Regulation on Biocidal
Products No. 528/2012): no"
Storage:
Store in a cool, dry and dark place; storage temperature: +5°C
to +25°C
The product considered in this EPD contains individual
components in the following ranges:
Shelf life:
18 months in standard cartridge systems
18 months in foil tube cartridge systems
Resin component:
Vinyl ester resin: 30 to 40% by weight
Gel and working time:
Mineral fillers: 50 to 70% by weight
-10°C 90 min.
Other components: < 5% by weight
-5°C 90 min.
0°C 45 min.
2 Environmental Product Declaration - MKT Metall-Kunststoff-Technik GmbH&Co. KG - VMU plus
Curing agent component: expected reference service life depends on the specific
Dibenzoyl peroxide: 10 to 15% by weight installation situation and on the product's resulting exposure.
Mineral fillers: 40 to 60% by weight The main factors influencing service life are weather conditions
Other components: 10 to 35% by weight and mechanical and chemical stresses.
Reference service life
The declared product VMU plus may be exposed to a wide
range of environmental conditions during the use phase. Its
LCA: Calculation rules
Declared Unit
The product declared is a two-component reaction resin mortar The precursor products are sourced from Germany, England
manufactured by MKT Metall-Kunststoff-Technik GmbH&Co. and France, Transport is mainly done by truck. Only the
KG with the product name VMU plus. The declared unit is transport from England is done by rail. The following process
based on 1 kg reaction resin product in the ratio at which the diagrams illustrate the underlying production process.
two components must be mixed before use.
The mixing ratio between the resin component and the curing
agent component is 9:1 [m/m] (volume ratio 10:1). The
packaging is also included in the calculation at 0.3013 kg per 1
kg of reaction resin product. The declared unit data are
presented in the table below.
Declared unit data
Name Value Unit
Declared unit 1 kg
Gross density 1770 kg/m3
Other declared units are allowed if the conversion is shown
transparently.
System boundary
Type of EPD: Cradle to factory gate with options. The following Figure 1 Information modules A 1 to A3 of the product
information modules are defined as system boundaries in this
study:
Production stage (A1- A3):
• A1, Raw material extraction,
• A2, Transport to the manufacturer,
Figure 2 Information modules A 1 to A3 of the packaging
• A3, Manufacturing.
Geographic Representativeness
End of life (C1- C4):
Land or region, in which the declared product system is
C1, Deconstruction/demolition,
manufactured, used or handled at the end of the product´s
C2, Transport,
lifespan: Germany
C3, Waste processing,
C4, Disposal.
Comparability
Reuse, recovery and recycling potential (D) Basically, a comparison or an evaluation of EPD data is only
possible if all the data sets to be compared were created
To precisely determine the indicators and environmental according to EN 15804 and the building context, respectively
impacts of the declared unit, a total of 8 information modules the product-specific characteristics of performance, are taken
are considered. The information modules A1 to A3 describe the into account.
material provision, the transport to the production site, as well
as the production processes of the product itself.
LCA: Scenarios and additional technical information
Name Value Unit
Characteristic product properties of biogenic carbon
Packaging PP 0.0318 kg
No renewable raw materials are used in the product or the
Packaging PA6 0.2696 kg
packaging. The biogenic carbon value is therefore reported as
zero.
Packaging per declared unit End of Life (C1-C4)
The product is demolished by using an electric chisel. The
electrical energy consumption for this tool is estimated at 0.05
3 Environmental Product Declaration - MKT Metall-Kunststoff-Technik GmbH&Co. KG - VMU plus
MJ for the declared unit. The power consumption is calculated
Reuse, recovery and recycling potential (D), relevant
using a European energy mix. Construcion waste is transported
scenario specifications
200 km by truck to a waste treatment facility. At the waste
The product has no reuse, recovery or recycling potential.
treatment facility, the construction waste is shredded and the
Information module D is therefore declared and reported as
disposed of in a landfill.
zero.
Name Value Unit
Name Value Unit
Reuse, recovery and recycling potential 0 kg
Collected as mixed construction waste 1 kg
Shredding 1 kg
Disposal in landfill 1 kg
4 Environmental Product Declaration - MKT Metall-Kunststoff-Technik GmbH&Co. KG - VMU plus
LCA: Results
DESCRIPTION OF THE SYSTEM BOUNDARY (X = INCLUDED IN LCA; MND = MODULE OR INDICATOR NOT DECLARED; MNR
= MODULE NOT RELEVANT)
Benefits and
Construction loads beyond
Product stage Use stage End of life stage
process stage the system
boundaries
la ire ta m w a Ry lp p u s tro p s n a rT g n iru tc a fu n a M e h t m o rf tro p s n a rTe tis e h t o t e ta g y lb m e s s A e s U e c n a n e tn ia M ria p e R tn e m e c a lp e R tn e m h s ib ru fe R y g re n e la n o ita re p Oe s u re ta w la n o ita re p Oe s u n o itc u rts n o c -e Dn o itilo m e d tro p s n a rT g n is s e c o rp e ts a W la s o p s iD -e s u e R-y re v o c e R-g n ilc y c e Rla itn e to p
A1 A2 A3 A4 A5 B1 B2 B3 B4 B5 B6 B7 C1 C2 C3 C4 D
X X X MND MND MND MND MNR MNR MNR MND MND X X X X X
RESULTS OF THE LCA - ENVIRONMENTAL IMPACT according to EN 15804+A2: 1 kg VMU plus
Parameter Unit A1-A3 C1 C2 C3 C4 D
Global Warming Potential total (GWP-total) kg CO 2 eq 4.68E+00 5.12E-03 1.51E-02 2.6E-03 1.45E-02 0
Global Warming Potential fossil fuels (GWP-fossil) kg CO 2 eq 4.68E+00 5.12E-03 1.5E-02 2.59E-03 1.45E-02 0
Global Warming Potential biogenic (GWP-biogenic) kg CO 2 eq 0 0 0 0 0 0
Global Warming Potential luluc (GWP-luluc) kg CO 2 eq 8E-04 1.08E-06 8.28E-05 1.2E-05 2.67E-05 0
Depletion potential of the stratospheric ozone layer (ODP) kg CFC11 eq 6.24E-09 7.5E-14 8.9E-16 3.85E-15 3.4E-14 0
Acidification potential of land and water (AP) mol H+ eq 7.09E-03 1.12E-05 4.67E-05 1.34E-05 1.03E-04 0
Eutrophication potential aquatic freshwater (EP-freshwater) kg P eq 2.57E-05 1.49E-08 4.43E-08 7.43E-09 2.45E-08 0
Eutrophication potential aquatic marine (EP-marine) kg N eq 2.29E-03 2.52E-06 2.15E-05 6.11E-06 2.62E-05 0
Eutrophication potential terrestrial (EP-terrestrial) mol N eq 2.1E-02 2.65E-05 2.4E-04 6.74E-05 2.88E-04 0
Formation potential of tropospheric ozone photochemical oxidants kg NMVOC
6.57E-03 6.82E-06 4.22E-05 1.66E-05 7.97E-05 0
(POCP) eq
Abiotic depletion potential for non fossil resources (ADPE) kg Sb eq 1.14E-06 1.4E-09 1.24E-09 2.87E-09 1.48E-09 0
Abiotic depletion potential for fossil resources (ADPF) MJ 9.01E+01 9.29E-02 1.98E-01 5.06E-02 1.9E-01 0
m3 world eq
Water use (WDP) 1.49E-01 1.17E-03 1.33E-04 4.99E-04 1.59E-03 0
deprived
RESULTS OF THE LCA - INDICATORS TO DESCRIBE RESOURCE USE according to EN 15804+A2: 1 kg VMU plus
Parameter Unit A1-A3 C1 C2 C3 C4 D
Renewable primary energy as energy carrier (PERE) MJ 1.17E+01 5.16E-02 1.13E-02 4.06E-03 2.85E-02 0
Renewable primary energy resources as material utilization
MJ 0 0 0 0 0 0
(PERM)
Total use of renewable primary energy resources (PERT) MJ 1.17E+01 5.16E-02 1.13E-02 4.06E-03 2.85E-02 0
Non renewable primary energy as energy carrier (PENRE) MJ 6.07E+01 9.3E-02 1.99E-01 5.07E-02 1.9E-01 0
Non renewable primary energy as material utilization (PENRM) MJ 2.95E+01 0 0 0 0 0
Total use of non renewable primary energy resources (PENRT) MJ 9.02E+01 9.3E-02 1.99E-01 5.07E-02 1.9E-01 0
Use of secondary material (SM) kg 0 0 0 0 0 0
Use of renewable secondary fuels (RSF) MJ 0 0 0 0 0 0
Use of non renewable secondary fuels (NRSF) MJ 0 0 0 0 0 0
Use of net fresh water (FW) m3 1.33E-02 4.92E-05 1.28E-05 1.42E-05 4.82E-05 0
RESULTS OF THE LCA – WASTE CATEGORIES AND OUTPUT FLOWS according to EN 15804+A2:
1 kg VMU plus
Parameter Unit A1-A3 C1 C2 C3 C4 D
Hazardous waste disposed (HWD) kg 9.76E-09 8.04E-12 9.53E-13 6.34E-13 9.75E-12 0
Non hazardous waste disposed (NHWD) kg 8.53E-02 7E-05 2.85E-05 1.34E-05 9.71E-01 0
Radioactive waste disposed (RWD) kg 1.33E-03 1.49E-05 2.45E-07 6.68E-07 2.11E-06 0
Components for re-use (CRU) kg 0 0 0 0 0 0
Materials for recycling (MFR) kg 0 0 0 0 0 0
Materials for energy recovery (MER) kg 0 0 0 0 0 0
Exported electrical energy (EEE) MJ 0 0 0 0 0 0
Exported thermal energy (EET) MJ 0 0 0 0 0 0
RESULTS OF THE LCA – additional impact categories according to EN 15804+A2-optional:
1 kg VMU plus
Parameter Unit A1-A3 C1 C2 C3 C4 D
Disease
Incidence of disease due to PM emissions (PM) ND ND ND ND ND ND
incidence
Human exposure efficiency relative to U235 (IR) kBq U235 eq ND ND ND ND ND ND
Comparative toxic unit for ecosystems (ETP-fw) CTUe ND ND ND ND ND ND
Comparative toxic unit for humans (carcinogenic) (HTP-c) CTUh ND ND ND ND ND ND
Comparative toxic unit for humans (noncarcinogenic) (HTP-nc) CTUh ND ND ND ND ND ND
5 Environmental Product Declaration - MKT Metall-Kunststoff-Technik GmbH&Co. KG - VMU plus
Soil quality index (SQP) SQP ND ND ND ND ND ND
The dataset "DE: Epoxy Resin, Source: Sphera, Reference year: 2021" was updated with reference to the previous EPD. As this
dataset has a strong influence on the overall calculation, the results are higher in comparison to the previous EPD from 2015.
References
Standards ETA-13/0909
European Technical Assessment.
DIN 51757
DIN 51757:2011-01 Testing of mineral oils and related ETA-11/0514
materials - Determination of density European Technical Assessment.
EN 196 IBU 2021
DIN EN 196-1:2016-11 Test methods for cement - Part 1: Institut Bauen und Umwelt e.V.: General guidance for the EPD
Determination of strength German version EN 196-1:2016 programme of the Institut Bauen und Umwelt e.V., Version 2.0,
Berlin: Institut Bauen und Umwelt e.V., 2021. www.ibu-epd.com
EN 15804
EN 15804:2019-04+A2, Sustainability of construction works - PCR PART A
Environmental Product Declarations - Core rules for the product Product Category Rules for Building-Related Products and
category of construction products. Services - Calculation Rules for the Life Cycle Assessment and
requirements on the Project Report V2.1, Institut Bauen und
ISO 14025 Umwelt e.V., 11.2021.
DIN EN ISO 14025:2011-10, Environmental labels and
declarations - Type III environmental declarations - Principles PCR: Reaction resin products
and procedures. Guidance-Texts for Building-Related Products and Services.
Part B: Requirements on the EPD for Reaction resin products,
ISO 14044 Version 1.3. Berlin: Institut Bauen und Umwelt e.V.
DIN EN ISO 14044:2006-10, Environmental management - Life (Hrsg.),07.2014.
cycle assessment - Requirements and guidelines.
Sphera
Further references GaBi 10 Software: Life Cycle Assessment Leinfelden-
Echterdingen; Sphera Solution GmbH (Hrsg.). http://www.gabi-
ecoinvent 3.7.1 software.com/deutsch/index/ (25/03/2022)
Background database: ecoinvent 3.7.1 Zürich: ecoinvent (Ed.) .
http://www.ecoinvent.org (25/03/2022) Regulation (EU) No. 305/2011
(CPR)
ETA-11/0415
European Technical Assessment. Regulation (EU) No. 528/2012
(Biocidal Product Regulation)
6 Environmental Product Declaration - MKT Metall-Kunststoff-Technik GmbH&Co. KG - VMU plus
Publisher
Institut Bauen und Umwelt e.V. +49 (0)30 3087748- 0
Hegelplatz 1 info@ibu-epd.com
10117 Berlin www.ibu-epd.com
Germany
Programme holder
Institut Bauen und Umwelt e.V. +49 (0)30 3087748- 0
Hegelplatz 1 info@ibu-epd.com
10117 Berlin www.ibu-epd.com
Germany
Author of the Life Cycle Assessment
FIT-Umwelttechnik GmbH 05362 72 69 474
Westerstr. 13 bertram@fit-umwelttechnik.de
38442 Wolfsburg www.fit-umwelttechnik.com
Germany
Owner of the Declaration
MKT Metall-Kunststoff-Technik GmbH & Co. KG +49 6374 9116-0
Auf dem Immel 2 info@mkt.de
67685 Weilerbach www.mkt.de
Germany
7 Environmental Product Declaration - MKT Metall-Kunststoff-Technik GmbH&Co. KG - VMU plus
