Environmental Product
Declaration
In accordance with ISO 14025 and EN 15804 +A2
Owner of the declaration: Wafix PP
Norsk Wavin AS
Program holder and publisher:
Wafix PP system is made from the
The Norwegian EPD foundation
PP (Polypropylene), which gives
both pipes and fittings good
Declaration number: physical and chemical properties.
NEPD-3587-2251-EN
Registration Number: Manufacturer
NEPD-3587-2251-EN
The Norwegian EPD AB Svenska Wavin
Foundation
Issue date: 16.08.2022
Valid to: 16.08.2027
Ver2-101122
General information
Product: Owner of the declaration:
Wafix PP pipe BK, GY, WT or BR with or without Norsk Wavin AS
socket, chamfered, plain; DN32, 40, 50, 75, 90, Contact person: Matteo Tagliaferri
110, 125, 160, 200. Phone: +31 623193684
e-mail: matteo.tagliaferri@wavin.com
Program Operator:
The Norwegian EPD Foundation Manufacturer:
Post Box 5250 Majorstuen, 0303 Oslo, Norway AB Svenska Wavin
Tlf: +47 23 08 80 00 Kjulamon 6, 635 06, Eskilstuna, Sweden
e-mail: post@epd-norge.no Phone: +46 (0) 16 541 00 00
e-mail: kundservice.se@wavin.com
Declaration Number:
NEPD-3587-2251-EN Place of production:
Kjulamon 6, 635 06, Eskilstuna, Sweden
This declaration is based on Product
Category Rules: Management system:
CEN standard EN 15804:2012+A2:2019 serves as EN ISO 9001:2015 and EN ISO 14001:2015
core PCR, supplied with NPCR Part A, Version 2.0.
Organization no:
Statements: 823355092
The owner of the declaration shall be liable for the
underlying information and evidence. EPD Issue date:
Norway shall not be liable with respect to 16.08.2022
manufacturer, life cycle assessment data and
evidences.
Valid to:
16.08.2027
Declared unit:
1 kg Wafix PP Pipe
Year of study:
2020
Declared unit with option:
A1,A2,A3,A4,A5,C1,C2,C3,C4,D
Comparability:
EPDs from other programmes than the Norwegian
Functional unit:
EPD foundation may not be comparable.
Not applicable.
The EPD has been worked out by:
Verification:
Lisa Overmars and Emma Thunnissen,
Independent verification of the declaration and
Ecochain Technologies
data, according to ISO14025:2010
internal external
Approved (Manager of EPD Norway)
Harry van Ewijk, SGS Search
Independent verifier approved by EPD Norway
EPD for the best environmental decision 2
Product
Product description:
The Wafix PP system is made from the recyclable PP (Polypropylene), which gives both pipes
and fittings good physical and chemical properties. The PP material used has a high E-module,
which gives the pipes a good length stiffness and a large impact strength. That is why the Wafix
PP system can withstand both large internal and external loads during assembly and
installation - even at minus degrees. The covered diameters are described in the Technical Data
section.
Product specification:
A typical composition of the pipes covered by this EPD is as follows:
Materials %
PP 98,5%
Additives 1,0%
Rubber gasket 0,1%
Packaging 0,4%
The physical properties of the pipes covered in this EPD are:
• Pipe material: Polypropylene (PP-B)
• Density ~ 901 kg/m³
• E-Modul ~ 1.800 Mpa
• Expansion linear ~ 0,15 mm/mK
• Thermal Conductivity w / 20 °C: 0.24 W / mK
• Operating temperature: 90°C
• Short-term peak temperature: 100° C (< 30 ltr/min in 2 min.)
The color of the pipe is either black (BK, RAL 9005), gray (GY, RAL 7037), white (WT, RAL
9003) or brown (BR, RAL 8012).
Technical data:
The declared unit of this EPD is 1 kg Wafix PP Pipe. The results per kg are based on the product
‘Wafix PP Pipe BR 110 SN8 L=6’ (‘base product’). The number 110 in the product name refers to
the diameter, which is equal to 110 mm. It follows that the pipe diameters can be derived from
the product names by taking the number after the color abbreviations.
The table below provides the products covered with this EPD. The selected base product is
representative for all products described in this table; deviations of the LCA results of the other
products compared to the base product are not more than 10%.
The list below provides the mass per 1 meter pipe (including packaging). These masses should
be used to calculate the LCA results per 1 meter pipe, by multiplying the results presented on
page 8-11 with the weight specified below.
EPD for the best environmental decision 3
Mass Mass
Product Product
(kg/meter) (kg/meter)
Wafix PP Pipe WT 32 L=1 S/CH 0,17 Wafix PP Pipe GY 75 L=4 PL/CH 0,53
Wafix PP Pipe WT 32 L=2 w/socket 0,17 Wafix PP Pipe GY 75 L=3 PL/CH 0,53
Wafix PP Pipe WT 32 L=3 PL/CH 0,17 Wafix PP Pipe GY 75 L=3 S/CH 0,53
Wafix PP Pipe WT 32 L=3 S/CH 0,17 Wafix PP Pipe GY 75 L=2 S/CH 0,53
Wafix PP Pipe GY 32 L=3 PL/CH 0,17 Wafix PP Pipe GY 75 L=1,5 S/CH 0,54
Wafix PP Pipe GY 32 L=2 S/CH 0,17 Wafix PP Pipe GY 75 L=1 S/CH 0,54
Wafix PP Pipe GY 32 L=1 S/CH 0,17 Wafix PP Pipe GY 75 L=0,5 S/CH 0,54
Wafix PP PipeWT 32 L=0,5 w/socket 0,17 Wafix PP Pipe BK 75 L=5 0,67
Wafix PP Pipe GY 32 L=1,5 S/CH 0,17 Wafix PP Pipe BK 75 L=3 0,67
Wafix PP Pipe GY 32 L=0,5 S/CH 0,18 Wafix PP Pipe BK 90 L=1 0,80
Wafix PP Pipe WT 32x3,0 L=4 0,27 Wafix PP Pipe BK 90 L=3 0,81
Wafix PP Pipe BK 32 L=3 0,27 Wafix PP Pipe BK 90 L=5 0,81
Wafix PP Pipe BK 32 L=5 0,28 Wafix PP Pipe BK 110 L=1 w/socket 1,13
Wafix PP Pipe WT 40 L=1 S/CH 0,22 Wafix PP Pipe BK 110 L=6 w/socket 1,13
Wafix PP Pipe WT 40 L=2 S/CH 0,22 Wafix PP Pipe BK 110 L=3 wo/socket 1,13
Wafix PP Pipe WT 40 L=3 S/CH 0,22 Wafix PP Pipe BK 110 L=3 w/socket 1,13
Wafix PP Pipe GY 40 L=3 PL/CH 0,22 Wafix PP Pipe GY 110 L=2 S/CH 1,13
Wafix PP Pipe WT 40 L=0,5 S/CH 0,22 Wafix PP Pipe GY 110 L=1,5 S/CH 1,13
Wafix PP Pipe GY 40 L=1,5 S/CH 0,22 Wafix PP Pipe GY 110 L=0,5 S/CH 1,13
Wafix PP Pipe GY 40 L=2 S/CH 0,22 Wafix PP Pipe GY 110 L=6 PL/CH 1,13
Wafix PP Pipe GY 40 L=1,25 S/CH 0,22 Wafix PP Pipe GY 110 L=6 S/CH 1,13
Wafix PP Pipe GY 40 L=1 S/CH 0,22 Wafix PP Pipe BK 110 L=5 1,13
Wafix PP Pipe GY 40 L=0,5 S/CH 0,22 Wafix PP Pipe GY 110 L=5 w/socket 1,13
Wafix PP Pipe WT 40x3,0 L=4 0,34 Wafix PP Pipe GY 110 L=4 S/CH 1,13
Wafix PP Pipe BK 40 L=5 0,34 Wafix PP Pipe BK 110 L=3 1,13
Wafix PP Pipe BK 40 L=3 0,34 Wafix PP Pipe GY 110 L=3 S/CH 1,13
Wafix PP Pipe WT 50 L=3 S/CH 0,28 Wafix PP Pipe GY 110 L=1 S/CH 1,14
Wafix PP Pipe WT 50 L=3 PL/CH 0,28 Wafix PP Pipe BR 110 SN8 L=6 1,28
Wafix PP Pipe GY 50 L=2 w/socket 0,28 Wafix PP Pipe BR 110 SN8 L=3 1,28
Wafix PP Pipe L/GY 50 L=3 w/socket 0,28 Wafix PP Pipe BR 110 SN8 L=2 1,28
Wafix PP Pipe GY 50 L=6 wo/socket 0,28 Wafix PP Pipe BR 110 SN8 L=1 1,29
Wafix PP Pipe WT 50 L=1 S/CH 0,28 Wafix PP Pipe BK 125 L=5 1,46
Wafix PP Pipe L/GY 50 L=1 0,28 Wafix PP Pipe GY 160 L=6 w/socket 2,34
Wafix PP Pipe L/GY 50 L=3 wo/socket 0,28 Wafix PP Pipe BK 160 L=5 2,34
Wafix PP Pipe GY 50 L=1,5 w/socket 0,28 Wafix PP Pipe GY 160 L=3 w/socket 2,34
Wafix PP Pipe WT 50 L=0,5 S/CH 0,28 Wafix PP Pipe GY 160 L=1 w/socket 2,36
Wafix PP Pipe GY 50 L=0,5 0,28 Wafix PP Pipe BR 160 SN8 L=6 2,66
Wafix PP Pipe WT 50x3,0 L=5 0,44 Wafix PP Pipe BR 160 SN8 L=3 2,67
Wafix PP Pipe BK 50 L=3 0,44 Wafix PP Pipe BR 160 SN8 L=2 2,67
EPD for the best environmental decision 4
Wafix PP Pipe BK 50 L=5 0,44 Wafix PP Pipe BR 160 SN8 L=1 S/CH 2,68
Wafix PP Pipe BK 75 L=1 w/socket 0,53 Wafix PP Pipe BR 200 SN8 L=6 4,16
Wafix PP Pipe BK 75 L=3 wo/socket 0,53 Wafix PP Pipe BR 200 SN8 L=3 4,17
Wafix PP Pipe BK 75 L=3 w/socket 0,53 Wafix PP Pipe BR 200 SN8 L=1 4,19
Wafix PP Pipe GY 75 L=6 PL/CH 0,53
Market:
Europe, but the EPD is specific for Nordic countries.
Reference service life, product:
Lifetime on product calculated is 100 year.
Reference service life, building:
Equal to building service life.
LCA: Calculation rules
Declared unit:
1 kg Wafix PP Pipe
Data quality:
For module A1, specific data for product compositions as provided by the manufacturer are
used. For module A2, transportation data of the raw materials used to the production site was
collected. For module A3, energy consumption and waste production data was collected for
production year 2020. The used background processes are derived from Ecoinvent 3.6.
Allocation:
Allocation was carried out in accordance with the provisions of the EN15804. All manufacturing
inputs (energy and auxiliary materials) at production site level are allocated to different
production processes, followed by allocation of the production processes to the products that
are produced using these processes through mass allocation. No secondary materials have been
used in the production process.
System boundary:
Modules A1-A5 and C1-D are included. The figure below shows a (simplified) process tree.
EPD for the best environmental decision 5
Cut-off criteria:
All relevant inputs and outputs - like emissions, energy and materials - have been taken into
account in this LCA. In accordance with EN15804, the total neglected input flows per module
does not exceed 5% of energy usage and mass.
EPD for the best environmental decision 6
LCA: Scenarios and additional technical information
The following information describe the scenarios in the different modules of the EPD.
Transport from production place to assembly/user (A4)
The transportation distance from Twist to Oslo was considered.
Capacity utilisation
Type Type of vehicle Distance KM Fuel/Energy consumption
(incl. return) %
Truck 50% Unspecified 422 0,027 l diesel/tkm
Assembly (A5)
Product losses of 10% are considered. The installation is done manually, and therefore no
energy is needed.
Unit Value
Material loss kg 0,1
Output materials from waste treatment kg 0,004
End of Life (C1, C3, C4)
Demolition is done manually, and therefore no energy is needed. The considered waste
treatment for the pipe is 70% recycling, 20% incineration and 10% landfill.
Unit Value
Collected as mixed construction waste kg 1,00
Reuse kg 0
Recycling kg 0,70
Energy recovery kg 0,20
To landfill kg 0,10
Transport to waste processing (C2)
The considered distances are 50 km to landfill, 100 km for energy recovery, and 250 km for
recycling.
Capacity utilisation
Type Type of vehicle Distance KM Fuel/Energy consumption
(incl. return) %
Truck 50% Unspecified 200,0 0,027 l diesel/tkm
Benefits and loads beyond the system boundaries (D)
For the PP, chemicals and additives, 0,67 kg of saved virgin PP was considered per kg material
recycled (total of A5 en C3). The benefits from exported energy were calculation from the
energy efficiencies for Northern countries reported by CEWEP, which is equal to an electrical
efficiency of 11,0%, and a thermal efficiency of 72,6%. Energy recovery from all materials
EPD for the best environmental decision 7
(including rubber gasket and packaging) was considered. Substition of Norwegian electricity
mix and district heating mix was assumed.
Unit Value
Saving of virgin PP kg 0.51
Substition of electric energy MJ 0,79
Subsitition of thermal energy MJ 5,18
Additional technical information
Not applicable.
LCA: Results
The LCA results are presented below for the declared unit defined on page 2 of the EPD
document. Recalculation to pipes with different diameters and lengths can be done based on the
technical data specified on page 3 and 4.
System boundaries (X=included, MND= module not declared, MNR=module not
relevant)
Benefits
& loads
Assembly
Product stage Use stage End of life stage beyond
stage
system
boundary
n -
s la ir e wt a am R t r o p s n a r T g n ir u t c a fu n a M t r o p s n a r T y lb m e s s A e s U e c n a n e t n ia M r ia p e R t n e m e c a lp e R t n e m h s ib r u fe R la n o ity ag rr eee pns Ou e la n o it ar re ete a ps w Ou n o io t cit ui rlo t sm ne od
c
-
t r o p s n a r T g n is s ee tc so ar Wp la s o p s iD g yn r eil v ec soy uc ce e RR --la it n e t o p
e e
D R
A1 A2 A3 A4 A5 B1 B2 B3 B4 B5 B6 B7 C1 C2 C3 C4 D
X X X X X X X X X X
Core environmental impact indicators
Indicator Unit A1-A3 A4 A5 C1 C2 C3 C4 D
GWP-total kg CO2 eq. 2,29E+00 5,52E-02 3,14E-01 0.00E+00 2,62E-02 7,60E-01 1,24E-02 -1,47E+00
GWP-fossil kg CO2 eq. 2,26E+00 5,51E-02 3,12E-01 0.00E+00 2,62E-02 7,61E-01 1,24E-02 -1,46E+00
GWP-
kg CO2 eq. 2,33E-02 3,35E-05 2,22E-03 0.00E+00 1,59E-05 -1,05E-03 1,08E-05 -4,70E-03
biogenic
GWP-LULUC kg CO2 eq. 6,74E-03 1,95E-05 6,91E-04 0.00E+00 9,28E-06 1,47E-04 2,10E-07 -2,60E-04
ODP kg CFC11 eq. 8,65E-08 1,27E-08 1,25E-08 0.00E+00 6,04E-09 1,91E-08 3,10E-10 -7,28E-08
AP mol H⁺ eq. 8,79E-03 3,14E-04 1,01E-03 0.00E+00 1,49E-04 8,04E-04 7,39E-06 -3,89E-03
EP-
kg P eq. 3,27E-05 4,54E-07 3,77E-06 0.00E+00 2,16E-07 4,24E-06 9,63E-09 -1,50E-05
freshwater
EPD for the best environmental decision 8
EP-marine kg N eq. 1,73E-03 1,12E-04 2,14E-04 0.00E+00 5,34E-05 2,33E-04 4,81E-06 -6,94E-04
EP-terrestial mol N eq. 1,94E-02 1,24E-03 2,39E-03 0.00E+00 5,89E-04 2,57E-03 3,00E-05 -7,69E-03
kg NMVOC
POCP 7,90E-03 3,54E-04 9,27E-04 0.00E+00 1,68E-04 8,13E-04 1,13E-05 -3,52E-03
eq.
ADP-M&M kg Sb eq. 3,54E-05 1,43E-06 4,08E-06 0.00E+00 6,78E-07 3,19E-06 7,44E-09 -8,90E-06
ADP-fossil MJ 7,49E+01 8,47E-01 7,88E+00 0.00E+00 4,02E-01 2,55E+00 2,26E-02 -4,41E+01
WDP m³ 1,76E+00 2,60E-03 1,81E-01 0.00E+00 1,23E-03 5,01E-02 1,13E-04 -7,35E-01
GWP-total: Global Warming Potential; GWP-fossil: Global Warming Potential fossil fuels; GWP-biogenic:
Global Warming Potential biogenic; GWP-LULUC: Global Warming Potential land use and land use change;
ODP: Depletion potential of the stratospheric ozone layer; AP: Acidification potential, Accumulated
Exceedance; EP-freshwater: Eutrophication potential, fraction of nutrients reaching freshwater end
compartment; See “additional Norwegian requirements” for indicator given as PO4 eq. EP-marine:
Eutrophication potential, fraction of nutrients reaching freshwater end compartment; EP-terrestial:
Eutrophication potential, Accumulated Exceedance; POCP: Formation potential of tropospheric ozone; ADP-
M&M: Abiotic depletion potential for non-fossil resources (minerals and metals); ADP-fossil: Abiotic
depletion potential for fossil resources; WDP: Water deprivation potential, deprivation weighted water
consumption
Additional environmental impact indicators
Indicator Unit A1-A3 A4 A5 C1 C2 C3 C4 D
Disease
PM 8,79E-08 4,98E-09 1,09E-08 0.00E+00 2,37E-09 1,32E-08 1,55E-10 -3,21E-08
incidence
IRP kBq U235 eq. 5,10E-02 3,70E-03 6,45E-03 0.00E+00 1,76E-03 7,69E-03 1,05E-04 -2,07E-02
ETP-fw CTUe 1,49E+01 6,87E-01 1,89E+00 0.00E+00 3,27E-01 2,88E+00 1,89E-02 -5,31E+00
HTP-c CTUh 6,67E-10 2,45E-11 1,05E-10 0.00E+00 1,16E-11 3,47E-10 5,52E-13 -2,35E-10
HTP-nc CTUh 1,80E-08 8,19E-10 2,37E-09 0.00E+00 3,89E-10 4,29E-09 1,22E-11 -5,67E-09
SQP Dimensionless 5,13E+00 7,24E-01 8,35E-01 0.00E+00 3,44E-01 2,04E+00 5,80E-02 -1,09E+00
PM: Particulate matter emissions; IRP: Ionising radiation, human health; ETP-fw: Ecotoxicity (freshwater);
ETP-c: Human toxicity, cancer effects; HTP-nc: Human toxicity, non-cancer effects; SQP: Land use related
impacts / soil quality
Classification of disclaimers to the declaration of core and additional environmental
impact indicators
ILCD
Indicator Disclaimer
classification
Global warming potential (GWP) None
ILCD type / level
Depletion potential of the stratospheric ozone layer (ODP) None
1
Potential incidence of disease due to PM emissions (PM) None
Acidification potential, Accumulated Exceedance (AP) None
Eutrophication potential, Fraction of nutrients reaching freshwater end
None
compartment (EP-freshwater)
ILCD type / level Eutrophication potential, Fraction of nutrients reaching marine end
None
2 compartment (EP-marine)
Eutrophication potential, Accumulated Exceedance (EP-terrestrial) None
Formation potential of tropospheric ozone (POCP) None
EPD for the best environmental decision 9
Potential Human exposure efficiency relative to U235 (IRP) 1
Abiotic depletion potential for non-fossil resources (ADP-minerals&metals) 2
Abiotic depletion potential for fossil resources (ADP-fossil) 2
Water (user) deprivation potential, deprivation-weighted water consumption
(WDP)
2
ILCD type / level
Potential Comparative Toxic Unit for ecosystems (ETP-fw) 2
3
Potential Comparative Toxic Unit for humans (HTP-c) 2
Potential Comparative Toxic Unit for humans (HTP-nc) 2
Potential Soil quality index (SQP) 2
Disclaimer 1 – This impact category deals mainly with the eventual impact of low dose ionizing radiation on
human health of the nuclear fuel cycle. It does not consider effects due to
possible nuclear accidents, occupational exposure nor due to radioactive waste disposal in underground facilities.
Potential ionizing radiation from the soil, from radon and from some
construction materials is also not measured by this indicator.
Disclaimer 2 – The results of this environmental impact indicator shall be used with care as the uncertainties on
these results are high or as there is limited experienced with the indicator
Resource use
Parameter Unit A1-A3 A4 A5 C1 C2 C3 C4 D
RPEE MJ 4,52E+00 1,21E-02 4,67E-01 0.00E+00 5,77E-03 1,26E-01 8,76E-04 -5,32E-01
RPEM MJ 0,00E+00 0,00E+00 0,00E+00 0.00E+00 0,00E+00 0,00E+00 0,00E+00 0,00E+00
TPE MJ 4,52E+00 1,21E-02 4,67E-01 0.00E+00 5,77E-03 1,26E-01 8,76E-04 -5,32E-01
NRPE MJ 8,04E+01 8,99E-01 8,45E+00 0.00E+00 4,27E-01 2,72E+00 2,40E-02 -4,76E+01
NRPM MJ 0,00E+00 0,00E+00 0,00E+00 0.00E+00 0,00E+00 0,00E+00 0,00E+00 0,00E+00
TRPE MJ 8,04E+01 8,99E-01 8,45E+00 0.00E+00 4,27E-01 2,72E+00 2,40E-02 -4,76E+01
SM kg 0,00E+00 0,00E+00 0,00E+00 0.00E+00 0,00E+00 0,00E+00 0,00E+00 0,00E+00
RSF MJ 0,00E+00 0,00E+00 0,00E+00 0.00E+00 0,00E+00 0,00E+00 0,00E+00 0,00E+00
NRSF MJ 0,00E+00 0,00E+00 0,00E+00 0.00E+00 0,00E+00 0,00E+00 0,00E+00 0,00E+00
W m3 2,95E-02 9,58E-05 3,12E-03 0.00E+00 4,55E-05 1,47E-03 2,79E-05 -1,09E-02
RPEE Renewable primary energy resources used as energy carrier; RPEM Renewable primary energy
resources used as raw materials; TPE Total use of renewable primary energy resources; NRPE Non
renewable primary energy resources used as energy carrier; NRPM Non renewable primary energy
resources used as materials; TRPE Total use of non renewable primary energy resources; SM Use of
secondary materials; RSF Use of renewable secondary fuels; NRSF Use of non renewable secondary fuels; W
Use of net fresh water
End of life - Waste
Parameter Unit A1-A3 A4 A5 C1 C2 C3 C4 D
HW KG 1,72E-05 2,16E-06 2,47E-06 0.00E+00 1,03E-06 4,15E-06 2,72E-08 -1,27E-05
NHW KG 2,69E-01 5,25E-02 5,74E-02 0.00E+00 2,49E-02 1,25E-01 9,97E-02 -3,34E-02
RW KG 5,40E-05 5,76E-06 7,26E-06 0.00E+00 2,74E-06 9,74E-06 1,48E-07 -1,93E-05
HW Hazardous waste disposed; NHW Non hazardous waste disposed; RW Radioactive waste disposed
EPD for the best environmental decision 10
End of life – output flow
Parameter Unit A1-A3 A4 A5 C1 C2 C3 C4 D
CR kg 0,00E+00 0,00E+00 2,14E-09 0.00E+00 0,00E+00 0,00E+00 0,00E+00 0,00E+00
MR kg 0,00E+00 0,00E+00 7,39E-02 0.00E+00 0,00E+00 6,97E-01 0,00E+00 0,00E+00
MER kg 0,00E+00 0,00E+00 1,99E-02 0.00E+00 0,00E+00 1,99E-01 0,00E+00 0,00E+00
EEE MJ 0,00E+00 0,00E+00 0,00E+00 0.00E+00 0,00E+00 0,00E+00 0,00E+00 5,18E+00
ETE MJ 0,00E+00 0,00E+00 0,00E+00 0.00E+00 0,00E+00 0,00E+00 0,00E+00 7,85E-01
CR Components for reuse; MR Materials for recycling; MER Materials for energy recovery; EEE Exported
electric energy; ETE Exported thermal energy
Information describing the biogenic carbon content at the factory gate
Biogenic carbon content Unit Value
Biogenic carbon content in product kg C 0
Biogenic carbon content in the accompanying packaging kg C 0
Additional Norwegian requirements
Greenhous gas emission from the use of electricity in the manufacturing phase
National production mix from import, low voltage (production of transmission lines, in addition
to direct emissions and losses in grid) of applied electricity for the manufacturing prosess(A3).
National electricity grid Unit Value
Hydroelectricity, average (Ecoinvent 3.6) kg CO2 -eq/kWh 0,0496
Additional environmental impact indicators required in NPCR Part A for construction
products
In order to increase the transparency of biogenic carbon contribution to climate impact, the
indicator for GWP has been sub-divided into the following:
GWP-IOBC Climate impacts calculated according to the principle of instantanious oxidation
GWP-BC Climate impacts from the net uptake and emission of biogenic carbon from each
module.
In addition, EP-freshwater shall also declared as PO4 eq.
Indicator Unit A1-A3 A4 A5 C1 C2 C3 C4 D
GWP-IOBC kg CO2 eq. 2,26E+00 5,52E-02 3,12E-01 0,00E+00 2,62E-02 7,61E-01 1,23E-02 -1,46E+00
GWP-BC kg CO2 eq. 2,33E-02 3,35E-05 2,22E-03 0,00E+00 1,59E-05 -1,05E-03 1,08E-05 -4,70E-03
GWP kg CO2 eq. 2,29E+00 5,52E-02 3,14E-01 0,00E+00 2,62E-02 7,60E-01 1,24E-02 -1,47E+00
EP-freshwater* Eutrophication potential, fraction of nutrients reaching freshwater end compartment.
Declared as PO4 eq. GWP-IOBC Global warming potential calculated according to the principle of
instantanious oxidation. GWP-BC Global warming potential from net uptake and emissions of biogenic
carbon from the materials in each module. GWP Global warming potential
EPD for the best environmental decision 11
Hazardous substances
The declaration is based upon reference to threshold values and/or test results and/or material
safety data sheets provided to EPD verifiers. Documentation available upon request to EPD
owner.
✓ The product contains no substances given by the REACH Candidate list or the
Norwegian priority list.
□ The product contains substances given by the REACH Candidate list or the Norwegian
priority list that are less than 0,1 % by weight.
□ The product contain dangerous substances, more then 0,1% by weight, given by the
REACH Candidate List or the Norwegian Priority list, see table.
□ The product contains no substances given by the REACH Candidate list or the
Norwegian priority list. The product is classified as hazardous waste (Avfallsforskiften,
Annex III), see table.
Indoor environment
The product meets the requirements for low emissions.
Carbon footprint
Carbon footprint has not been worked out for the product.
EPD for the best environmental decision 12
Bibliography
ISO 14025:2010 Environmental labels and declarations - Type III environmental
declarations - Principles and procedures
ISO 14044:2006 Environmental management - Life cycle assessment -
Requirements and guidelines
EN 15804:2012+A2:2019 Sustainability of construction works - Environmental product
declaration - Core rules for the product category of construction
products
ISO 21930:2007 Sustainability in building construction – Environmental
declaration of building products
NPCR Part A Construction products and services. Ver. 2.0. March 2021, EPD-
Norge
CEWEP Results of Specific Data for Energy, R1 Plant Efficiency Factor and
NCV of 314 European Waste-to-Energy (WtE) Plants, CEWEP
Energy Report III (status 2007-2010), 2012, Reiman, D.O.
Program Operator tlf +47 23 08 80 00
The Norwegian EPD Foundation
Post Box 5250 Majorstuen, 0303 Oslo e-post: post@epd-norge.no
Norway web www.epd-norge.no
Publisher tlf +47 23 08 80 00
The Norwegian EPD Foundation
Post Box 5250 Majorstuen, 0303 Oslo e-post: post@epd-norge.no
Norway web www.epd-norge.no
Owner of the declaration tlf +4745190625
Norsk Wavin AS Fax
Karihaugveien 89, 1086, Oslo e-post: Invoice.no@wavin.com
Norway web www.wavin.com/nn-no
Author of the life cycle assessment tlf +31 (0)20 303 5777
Lisa Overmars Fax
H.J.E. Wenckebachweg 123, 1096 AM
e-post: lovermars@ecochain.com
Amsterdam
The Netherlands web www.ecochain.com
EPD for the best environmental decision 13
EPD for the best
environmental
decision
The Norwegian EPD foundation
www.epd-norge.no
