ENVIRONMENTAL PRODUCT DECLARATION
as per ISO 14025 and EN 15804+A2
Owner of the Declaration IGI - The Global Wallcoverings Association
Publisher Institut Bauen und Umwelt e.V. (IBU)
Programme holder Institut Bauen und Umwelt e.V. (IBU)
Declaration number EPD-IGI-20230438-IBG1-EN
Issue date 18.01.2024
Valid to 17.01.2029
Wallcoverings on cellulose fibre base
IGI - The Global Wallcoverings Association
www.ibu-epd.com | https://epd-online.com
1. General Information
IGI - The Global Wallcoverings Association Wallcoverings on cellulose fibre base
Programme holder Owner of the declaration
IBU – Institut Bauen und Umwelt e.V. IGI - The Global Wallcoverings Association
Hegelplatz 1 Chaussée de Louvain 426
10117 Berlin 1380 LASNE
Germany Belgium
Declaration number Declared product / declared unit
EPD-IGI-20230438-IBG1-EN The declared unit is 1m² (square meter) decorative wallcovering on
cellulose fibre base including packaging.
This declaration is based on the product category rules: Scope:
Wall coverings, 01.08.2021 This EPD focusses on the production, transport and disposal of a weighted
(PCR checked and approved by the SVR) average of 1m² wallcoverings on cellulose fibre base of participating
members of the IGI - The Global Wallcoverings Association. Non-
decorative wallcoverings for a later additional treatment like painting
Issue date ("whites") are included in this scope as they follow a worst case approach.
13 out of 71 IGI-members are involved in this EPD: Anstey Wallpaper Co.
18.01.2024
Ltd (GB), A.S. Création Tapeten AG (DE), Borås Tapetfabrik AB (SE),
Decoprint NV (BE), Erfurt & Sohn KG (DE), Erismann & Cie. GmbH (DE),
Fine Decor Wallcoverings Ltd (GB), Flügger A/S (DK), Graham & Brown
Valid to
Ltd (GB), Grandeco NV (BE), Rasch GmbH & Co. KG (DE), UGÉPA SA
17.01.2029 (FR), York Wallcoverings inc. (US). The technical properties are displayed
in chapter 2.3.
The owner of the declaration shall be liable for the underlying information
and evidence; the IBU shall not be liable with respect to manufacturer
information, life cycle assessment data and evidences.
The EPD was created according to the specifications of EN 15804+A2. In
the following, the standard will be simplified as EN 15804.
Verification
The standard EN 15804 serves as the core PCR
Independent verification of the declaration and data according to ISO
Dipl.-Ing. Hans Peters
14025:2011
(Chairman of Institut Bauen und Umwelt e.V.)
internally X externally
Florian Pronold Prof. Dr. Birgit Grahl,
(Managing Director Institut Bauen und Umwelt e.V.) (Independent verifier)
1 Environmental Product Declaration - IGI - The Global Wallcoverings Association - Wallcoverings on cellulose fibre base
2. Product
Declaration of Performance with respect to its Essential
2.1 Product description/Product definition Characteristics according to EN 15102.
Wallcoverings on cellulose fibre base according to EN 15102
involve a cellulose fibre base. When the wallcovering is to be or:
changed, it can be removed from the wall by wetting the
surface, allowing moisture to penetrate the wallcovering, and 1b
then using a scraper for removal. This property as defined in Performance Category I, II, III, IV, V or VI as described in Table
EN 235 is wet removable. For the placing on the market of the 1 of F 793-0-06 should be declared.
product in the European Union/European Free Trade
Association (EU/EFTA) (with the exception of Switzerland) 2.4 Delivery status
Regulation (EU) No. 305/2011 (CPR) applies. The product The products declared are provided within the following
needs a Declaration of Performance taking into consideration dimensions:*
EN 15102 and CE-marking.
For the application and use the respective national provisions
apply.
For the placing on the market in Great Britain the product
needs a Declaration of Performance taking into consideration This table contains the range of all wallcoverings examined. For
BS EN 15102 and UK Conformity Assessed (UKCA) marking. more precise information please contact the specific
manufacturer.
For placing on the market in Northern Ireland the product needs
2.5 Base materials/Ancillary materials
a Declaration of Performance taking into consideration (BS) EN
The weighted average of the primary product components is
15102 and CE or CE and UK Northern Ireland (UKNI) marking.
shown in the following table, in percentage:
For the placing on the market in the USA the product should Name Value Unit
conform to ASTM F 1141 – 93 Standard Specification for Carrier material (Paper) 76 %
Wallcovering and ASTM F 793 – 06 Standard Classification of Packaging 13 %
Wall Covering by Use Characteristics.
Ink & Pigment 7 %
2.2 Application Additives 4 %
Wallcoverings are used for the decorative wall design of interior Sum 100 %
spaces in private or commercial use.
Pallets were considered as part of the packaging.
2.3 Technical Data
This product contains substances listed in the candidate list
In accordance with EN 233, the following technical (structural)
(date: 06.12.2023) exceeding 0.1 percentage by mass: no.
data can be declared on delivery:
This product contains other CMR substances in categories 1A
Constructional data or 1B that are not on the candidate list, exceeding 0.1
Name Value Unit percentage by mass: no.
Measures by categories EN 233 category 1 - 3 - Biocide products were added to this construction product or it
has been treated with biocide products (this then concerns a
Straightness and parallelism in mm.
equal or less than 1 - treated product as defined by the (EU) Ordinance on Biocide
according to EN 12956
Products No. 528/2012): no.
spongeable to
Washability according to EN 12956 - Ancillary materials of the phthalate chemical group, specifically
extra-washable
Diisononyl phthalate (DINP), remain on the product and serve
Colour fastness to light according to the function of softeners.
3 - 6 -
EN ISO 105-B02 This EPD is a weighted average of a Manufacturer Group
Migration of heavy metals and certain regarding several producers and product references. Therefore,
fulfills the norm -
other elements to EN 12149 it cannot be ruled out that individual wallcoverings may contain
Emissions of formaldehyde max. small amounts (>0.1% of product weight) of substances that
< 120 mg/kg according to EN 12149 fulfills the norm - are included in the Substance of Very High Concern SVHC
candidate list, the CMR substances in categories 1A or 1B list
or ancillary materials and additives serving the function of fire
This table contains the range of all wallcoverings examined. For
retardants, softeners or biocides.
more precise information please contact the specific
This can be attributed, for example, to the contents of used
manufacturer.
waste paper.
Further information can be obtained from the respective
For USA manufactured products should be in accordance with
manufacturer.
ASTM F 793-0-06 Table 1 Classification Criteria.
2.6 Manufacture
Depending on whether products are intended for the European, The manufacturing process can be described with the help of
UK or US market, the following performance data must be the following graphic:
declared.
1a: Product according to the CPR, based on (BS) EN
15102:
Performance data of the product in accordance with the
2 Environmental Product Declaration - IGI - The Global Wallcoverings Association - Wallcoverings on cellulose fibre base
Building Assessment System (BNB).
Description of the influences on the ageing of the product when
applied in accordance with the rules of technology.
2.13 Extraordinary effects
Fire
The reaction to fire performance according to EN 13501 is
shown in the following table:*
Name Value
Building material class B - D
Burning droplets s1 - s3
Smoke gas development d0 - d2
*This table contains the range of all wallcoverings examined.
For more precise information please contact the specific
The order of manufacture may change and can slightly deviate manufacturer.
for different producers.
For USA information on fire performance according to ASTM E
2.7 Environment and health during manufacturing 84 Test method for Surface Burning Characteristics of Building
Compliance with statutory health and safety for personnel is Materials.
ensured. Further, the energy and environmental management
is certified for some members according to ISO 14001 and ISO
50001. Water
For greater detail please contact the specific manufacturer. The product is not water resistant. There is no risk of a
hazardous environmental impact in the event of water flooding.
2.8 Product processing/Installation
Depending on the manufacturers suggestion, the adhesive is Mechanical destruction
applied to the back of the wallcovering or the substrate using a There is no risk of a hazardous environmental impact following
wallpaper brush or short-napped roller. The wallcovering is unforeseen mechanical destruction.
pressed against the wall and is cut along the top and bottom
edge to fit the wall. 2.14 Re-use phase
The product is not re-usable.
2.9 Packaging
The product is wrapped in clear shrink-wrap, packed in 2.15 Disposal
corrugated cardboard boxes and palletised. Wallcoverings are subject to the waste code 170904 (mixed
construction and demolition waste other than those mentioned
2.10 Condition of use
in 170901, 170902 and 170903) in accordance with the
There are no special features to be noted within the limits of European Waste Catalogue (EWC).
normal and customary usage. Wallcoverings can therefore be disposed of as normal
household waste, that is in the dustbin or in additional refuse
2.11 Environment and health during use
sacks. Used wallcoverings should not be placed in the waste
No environmental problems can be expected when the product
paper bank. Most household waste is incinerated or landfilled
is handled and used
depending on regional legal regulations in the EU or in the US.
properly.
2.16 Further information
2.12 Reference service life
For further information please visit www.igiwallcoverings.org.
Given the wallcovering is professionally installed, the reference
service life is 10 years according to the German Sustainable
3. LCA: Calculation rules
3.1 Declared Unit 3.2 System boundary
The declared unit is 1 m² of wallcovering including packaging. Type of the EPD: cradle to gate - with options.
The model is based on a weighted average of the produced The EPD is considered a declaration of an average product as
square meters of each participating manufacturer. calculated from the output of several manufacturers (2b).
Declared unit
Modules A1-3, A4 and A5
Name Value Unit
The product stage begins with the consideration of the
Declared unit 1 m2 production of the necessary raw materials and energies
Grammage 0.146 kg/m2 including all corresponding upstream processes as well as
transport.
Conversion factor to 1 kg 6.867 -
Furthermore, the entire production phase was investigated,
Layer thickness 0.001 m
including the treatment of production waste until reaching the
Density 1456 kg/m3 end-of-waste status (EoW). In addition, distribution transport
and installation in the building were taken into account.
The production processes and location may vary between
individual companies. The weighted average represents the
Modules C1-4
most likely scenario by production volumes and the selected
The modules include the environmental impacts of the removal
datasets correspond to all regarded regions.
and waste treatment until reaching the end-of-waste status
3 Environmental Product Declaration - IGI - The Global Wallcoverings Association - Wallcoverings on cellulose fibre base
(EoW) including the associated transport at the end of the environmental data, the collection of LCA-relevant data within
product life cycle. the supply chain as well as through the measurement of
relevant energy supply data. The collected data were checked
Module D for plausibility and consistency. A good representation is to be
Calculation of potential benefits through the generated energy assumed. The data were collected in 2022 and refer to the
(electric & thermic) by the incineration processes in the life calendar year 2021.
cycle stages in A5 C3 and C4. The burdens resulting from the
waste-to-energy plants are assigned in module C3 or C4 in 3.7 Period under review
case of landfill gas combustion. The LCA data were collected for the calendar year 2021.
3.3 Estimates and assumptions 3.8 Geographic Representativeness
Most solvents were modelled as a generic mix of solvents. Land or region, in which the declared product system is
manufactured, used or handled at the end of the product´s
3.4 Cut-off criteria lifespan: Global
No materials were cut-off from the study. No energy
consumption was neglected.
3.9 Allocation
3.5 Background data Potential benefits resulting from the thermal utilization of the
For modelling the lifecycle, the LCA for Experts Software packaging waste (module A5) as well as from the thermal
System and Database for Life Cycle Engineering (GaBi) utilization or landfilling of the wallcoverings at the end of life
Service pack 2023.1 was used. All background data records (modules C3 and C4) are allocated to module D.
relevant for production and disposal were almost exclusively
3.10 Comparability
taken from various GaBi supplementary databases or rarely
also from ecoinvent (v.3.6). The data records included in the Basically, a comparison or an evaluation of EPD data is only
databases are documented online. possible if all the data sets to be compared were created
according to EN 15804 and the building context, respectively
3.6 Data quality the product-specific characteristics of performance, are taken
Data collection for the investigated products was carried out on into account. The used background database is GaBi service
the basis of evaluations of the internal production and package 1 of 2023.
4. LCA: Scenarios and additional technical information
Characteristic product properties of biogenic carbon Modules B1-B7 are deemed not relevant since the product
The biogenic carbon content quantifies the amount of biogenic needs no maintenance or operational energy or water use and
carbon in a construction product leaving the factory gate, and it are are therefore, not declared.
is separately declared for the product and for any
accompanying packaging. 1 kg of biogenic Carbon is
Installation into the building (A5)
equivalent to 44/12 kg of CO .
2 The treatment of packaging as waste was modeled in Module
Information on describing the biogenic Carbon Content at A5 as a weighted average. The following table depicts the
factory gate packaging materials treated in A5 with more than 1 gram of
Name ValueUnit participation in the weighted average.
kg
Biogenic carbon content in product 0.04 Modules B1-B7 are deemed not relevant since the product
C
needs no maintenance or operational energy or water use and
Biogenic carbon content in accompanying kg
0.004 are are therefore, not declared.
packaging C
Name Value Unit
Note: 1 kg of biogenic carbon is equivalent to 44/12 kg of CO2.
Cardboard 0.009 kg
Pallet 0.005 kg
Polyethylene 0.005 kg
Paper 0.001 kg
Transport to the building site (A4)
Name Value Unit Reference service life
Truck transport 27 t payload Name Value Unit
Transport distance 413 km Reference service life 10 a
Train transport 726 t payload
End of life (C1-C4)
Transport distance 2 km
Ship transport 27500 dwt payload Name Value Unit
Transport distance 255 km Incineration 94 %
Cargo plane transport 65 t payload Landfilling 6 %
Transport distance 75 km For the calculation of this LCA landfilling is chosen for the US
Capacity utilisation (including empty runs) 80 - 90 % and incineration for the EU. Different disposal routes are
available but not taken into account for this industry average
Because many different countries are involved, there were
LCA.
always global data sets used to model the transport distances.
The benefits from thermal combustion of the wallcoverings are
The treatment of packaging as waste was modelled in Module
calculated in Module D. From the total paper used as backing,
A5 as a weighted average.
36.8% of recycled paper in product does not receive benefits,
4 Environmental Product Declaration - IGI - The Global Wallcoverings Association - Wallcoverings on cellulose fibre base
as it is a secondary material coming burden-free to the system. incineration of landfill gases (C4) are displayed.
In module D the potential benefits of the thermal combustion of
the wallcoverings (C3) and their packaging (A5) as well as the
5 Environmental Product Declaration - IGI - The Global Wallcoverings Association - Wallcoverings on cellulose fibre base
5. LCA: Results
In this section, the LCA results for 1 m² wallcoverings are presented. It should be borne in mind that the LCA results only indicate
possible effects.
Indicators used for evaluation:
The EN 15804+A2 LCIA methodology with the characterization factors from EK-JRC were used to evaluate the possible environmental
effects of the wallcoverings.
The characterization factors are available at the following internet link: http://eplca.jrc.ec.europa.eu/LCDN/developerEF.xhtml.
DESCRIPTION OF THE SYSTEM BOUNDARY (X = INCLUDED IN LCA; MND = MODULE OR INDICATOR NOT DECLARED; MNR
= MODULE NOT RELEVANT)
Benefits and
Construction loads beyond
Product stage Use stage End of life stage
process stage the system
boundaries
la ire ta m w a Ry lp p u s tro p s n a rT g n iru tc a fu n a M e h t m o rf tro p s n a rTe tis e h t o t e ta g y lb m e s s A e s U e c n a n e tn ia M ria p e R tn e m e c a lp e R tn e m h s ib ru fe R y g re n e la n o ita re p Oe s u re ta w la n o ita re p Oe s u n o itc u rts n o c -e Dn o itilo m e d tro p s n a rT g n is s e c o rp e ts a W la s o p s iD -e s u e R-y re v o c e R-g n ilc y c e Rla itn e to p
A1 A2 A3 A4 A5 B1 B2 B3 B4 B5 B6 B7 C1 C2 C3 C4 D
X X X X X MND MND MNR MNR MNR MND MND X X X X X
RESULTS OF THE LCA - ENVIRONMENTAL IMPACT according to EN 15804+A2: 1 m² wallcoverings on cellulose fibre base
Parameter Unit A1-A3 A4 A5 C1 C2 C3 C4 D
GWP-total kg CO 2 eq 1.71E-01 3.17E-02 2.75E-02 2.66E-05 1.19E-03 1.62E-01 8.68E-03 -6.36E-02
GWP-fossil kg CO 2 eq 3.33E-01 3.17E-02 1.45E-02 2.66E-05 1.18E-03 2.45E-02 5E-04 -6.36E-02
GWP-biogenic kg CO 2 eq -1.59E-01 0 1.3E-02 0 0 1.38E-01 8.18E-03 0
GWP-luluc kg CO 2 eq -2.85E-03 4.97E-05 1.5E-06 8.89E-09 1.09E-05 1.4E-06 4.12E-07 -4.1E-06
ODP kg CFC11 eq 8.53E-10 2.15E-15 2.14E-15 1.62E-16 1.53E-16 2.44E-14 7.62E-16 -4.94E-13
AP mol H+ eq 1.01E-03 1.55E-04 6.06E-06 6.73E-08 9.82E-06 4.92E-05 2.37E-06 -7.86E-05
EP-freshwater kg P eq 2.82E-05 2.37E-08 3.25E-08 2.34E-09 4.29E-09 8.22E-09 5.46E-08 -1.02E-07
EP-marine kg N eq 3.81E-04 6.9E-05 2.46E-06 2.36E-08 4.9E-06 1.79E-05 1.36E-06 -2.3E-05
EP-terrestrial mol N eq 3.74E-03 7.58E-04 2.75E-05 1.63E-07 5.41E-05 2.23E-04 8.47E-06 -2.46E-04
kg NMVOC
POCP 7.84E-04 1.8E-04 6.96E-06 4.41E-08 9.25E-06 4.74E-05 4.85E-06 -6.4E-05
eq
ADPE kg Sb eq 1.53E-07 6.12E-10 3.12E-11 1.53E-12 7.73E-11 2.19E-10 1.32E-11 -4.52E-09
ADPF MJ 5.92E+00 4.27E-01 1.01E-02 4.75E-04 1.6E-02 5.99E-02 6.95E-03 -1.16E+00
m3 world eq
WDP 3.34E-01 1.02E-04 2.32E-03 8.59E-03 1.42E-05 2.09E-02 3.15E-05 -5.98E-03
deprived
GWP = Global warming potential; ODP = Depletion potential of the stratospheric ozone layer; AP = Acidification potential of land and water; EP =
Eutrophication potential; POCP = Formation potential of tropospheric ozone photochemical oxidants; ADPE = Abiotic depletion potential for non-fossil
resources; ADPF = Abiotic depletion potential for fossil resources; WDP = Water (user) deprivation potential)
RESULTS OF THE LCA - INDICATORS TO DESCRIBE RESOURCE USE according to EN 15804+A2: 1 m² wallcoverings on
cellulose fibre base
Parameter Unit A1-A3 A4 A5 C1 C2 C3 C4 D
PERE MJ 3.34E+00 6.46E-03 2.22E-01 9.67E-05 1.16E-03 1.59E+00 9.41E-02 -3.37E-01
PERM MJ 1.89E+00 0 -2.2E-01 0 0 -1.57E+00 -9.35E-02 0
PERT MJ 5.23E+00 6.46E-03 1.54E-03 9.67E-05 1.16E-03 1.48E-02 6.35E-04 -3.37E-01
PENRE MJ 5.41E+00 4.29E-01 2.15E-01 4.75E-04 1.61E-02 3.59E-01 1.38E-02 -1.16E+00
PENRM MJ 5.1E-01 0 -2.05E-01 0 0 -2.99E-01 -6.85E-03 0
PENRT MJ 5.92E+00 4.29E-01 1.01E-02 4.75E-04 1.61E-02 5.99E-02 6.95E-03 -1.16E+00
SM kg 3.99E-02 0 0 0 0 0 0 0
RSF MJ 0 0 0 0 0 0 0 0
NRSF MJ 0 0 0 0 0 0 0 0
FW m3 7.79E-03 7.42E-06 5.48E-05 2E-04 1.27E-06 4.93E-04 9.6E-07 -2.73E-04
PERE = Use of renewable primary energy excluding renewable primary energy resources used as raw materials; PERM = Use of renewable primary
energy resources used as raw materials; PERT = Total use of renewable primary energy resources; PENRE = Use of non-renewable primary energy
excluding non-renewable primary energy resources used as raw materials; PENRM = Use of non-renewable primary energy resources used as raw
materials; PENRT = Total use of non-renewable primary energy resources; SM = Use of secondary material; RSF = Use of renewable secondary fuels;
NRSF = Use of non-renewable secondary fuels; FW = Use of net fresh water
RESULTS OF THE LCA – WASTE CATEGORIES AND OUTPUT FLOWS according to EN 15804+A2:
1 m² wallcoverings on cellulose fibre base
Parameter Unit A1-A3 A4 A5 C1 C2 C3 C4 D
HWD kg 1.4E-07 9.15E-13 4.63E-13 1.35E-14 4.97E-14 1.66E-12 5.89E-13 -6.19E-11
NHWD kg 9.64E-03 4.31E-05 3.22E-03 6.08E-05 2.45E-06 7.97E-03 5.83E-03 -5.73E-04
RWD kg 2.07E-04 4.59E-07 2.89E-07 1.9E-08 3E-08 3.05E-06 8.21E-08 -8.95E-05
6 Environmental Product Declaration - IGI - The Global Wallcoverings Association - Wallcoverings on cellulose fibre base
CRU kg 0 0 0 0 0 0 0 0
MFR kg 0 0 0 0 0 0 0 0
MER kg 1.05E-02 0 1.03E-02 0 0 1.18E-01 0 0
EEE MJ 2.47E-02 0 0 0 0 0 0 2.98E-01
EET MJ 4.33E-02 0 0 0 0 0 0 5.38E-01
HWD = Hazardous waste disposed; NHWD = Non-hazardous waste disposed; RWD = Radioactive waste disposed; CRU = Components for re-use;
MFR = Materials for recycling; MER = Materials for energy recovery; EEE = Exported electrical energy; EET = Exported thermal energy
RESULTS OF THE LCA – additional impact categories according to EN 15804+A2-optional:
1 m² wallcoverings on cellulose fibre base
Parameter Unit A1-A3 A4 A5 C1 C2 C3 C4 D
Disease
PM 1.46E-08 6.99E-10 4.14E-11 1.08E-12 6.98E-11 2.93E-10 2.3E-11 -6.67E-10
incidence
IR kBq U235 eq 8.42E-02 6.42E-05 4.55E-05 2.91E-06 4.48E-06 4.74E-04 1.21E-05 -1.49E-02
ETP-fw CTUe 8.58E+00 3.01E-01 7.01E-03 9.77E-04 1.14E-02 2.82E-02 6.41E-03 -2.54E-01
HTP-c CTUh 5.73E-10 5.62E-12 3.59E-13 1.86E-14 2.34E-13 1.65E-12 3.03E-13 -1.28E-11
HTP-nc CTUh 5.14E-08 3.04E-10 2.84E-11 1.74E-12 1.42E-11 8.6E-11 3.63E-11 -3.99E-10
SQP SQP 1.61E+01 3.12E-02 2.37E-03 7.06E-05 6.68E-03 1.71E-02 6.22E-04 -2.22E-01
PM = Potential incidence of disease due to PM emissions; IR = Potential Human exposure efficiency relative to U235; ETP-fw = Potential comparative
Toxic Unit for ecosystems; HTP-c = Potential comparative Toxic Unit for humans (cancerogenic); HTP-nc = Potential comparative Toxic Unit for humans
(not cancerogenic); SQP = Potential soil quality index
Disclaimer 1 – for the indicator “Potential Human exposure efficiency relative to U235”. This impact category deals mainly with the
eventual impact of low-dose ionizing radiation on human health of the nuclear fuel cycle. It does not consider effects due to possible
nuclear accidents, occupational exposure or radioactive waste disposal in underground facilities. Potential ionizing radiation from the
soil, radon and from some construction materials is also not measured by this indicator.
Disclaimer 2 – for the indicators “abiotic depletion potential for non-fossil resources”, “abiotic depletion potential for fossil resources”,
“water (user) deprivation potential, deprivation-weighted water consumption”, “potential comparative toxic unit for ecosystems”,
“potential comparative toxic unit for humans – cancerogenic”, “Potential comparative toxic unit for humans - not cancerogenic”,
“potential soil quality index”. The results of this environmental impact indicator shall be used with care as the uncertainties on these
results are high as there is limited experience with the indicator.
This EPD was created using a software tool.
6. LCA: Interpretation
7 Environmental Product Declaration - IGI - The Global Wallcoverings Association - Wallcoverings on cellulose fibre base
dioxide contained in the paper is treated first as a credit; after
The production stage (module A1-A3) clearly dominates the incineration in a waste-to-energy facility, it is treated as a load
LCA results. The loads caused by the disposal stage (modules (C3). Moreover, paper production has a relatively large
C3 and C4) become noticeable, especially as the biogenic influence on the acidification potential (AP), the eutrophication
carbon leaves the product system, reflected in the total and potential (EP), the ozone depletion (ODP), and the Potential for
biogenic global warming potential. Transports play a the formation of tropospheric ozone (POCP).
subordinate yet not insignificant role. The main environmental
impacts are in all categories located in module A1-A3. For Range of the results
GWP-fossil and ADPF the highest precursor of impact is the The individual results of the participating companies differ from
generation of thermal and electric energy for general production the average results in the present environmental product
and heating/drying processes in A3. Paper production, both declaration. Regarding GWP, the results may be 97% higher or
from primary and secondary sources, is the next highest source 61% lower than the average for this EPD.
of impact in the GWP-fossil category and ADPF. The main reason for the deviations is differences in the
grammage of the individual wallcoverings. In addition, there are
The production of recycled paper has a noticeable effect. It has different materials used as well as varying heat and electricity
a relatively high share of the greenhouse potential due to consumptions depending on the manufacturer.
energy demands. In the GWP category, the biogenic carbon
7. Requisite evidence
Members of the The Global Wallcoverings Association have the wallcoverings meet the requirements of test standard
following certificates: ISO 16000.
• Optional compliance with German RAL-GZ 479.
• The declared products comply with EN 15102.
• Optional compliance with USA Wallcovering Association
• According to the (emission) test chamber assessment,
W-101 (2013) paragraph 8.1 when tested by California
which follows the French measurement method Arrêté
Specification Section 01350 to criteria CDPH/EHLB
du 19/04/11 the wallcoverings meet the requirements of
Standard Method V1.1 (2010).
the test standard ISO 16000.
The certificates and classifications for the various wallcoverings
• Optional according to the chamber test which follows
can be obtained from the respective manufacturers.
the German AgBB (Committee for health-related
evaluation of building products) regulations the
8. References
Standards and Norms
EN 12956:1999
Arrêté du 19/04/11 Wallcoverings in roll form - Determination of dimensions,
Order of 19 April 2011 relating to the labeling of construction straightness, spongeability and washability.
products or wall or floor coverings and paints and varnishes on
their emissions of volatile pollutants EN 13501-1:2018
Fire classification of construction products and building
ASTM E 84 elements - Part 1: Classification using data from reaction to fire
ASTM E 84:2016: Standard Test Method for Surface Burning Tests.
Characteristics of Building Materials
EN 15102:2007+A1:2011
ASTM F 793 Decorative wallcoverings - Roll and panel form.
ASTM F793 / F793M-15, Standard Classification of Wall
Coverings by Use Characteristics, ASTM International, West EN 233:2016
Conshohocken, PA, 2015 Wallcoverings in roll form - Specification for finished wallpapers,
wall vinyls and plastics wallcoverings.
ASTM F1141 - 93
ASTM F1141-93(2009), Standard Specification for EN 234:2019
Wallcovering, ASTM International, West Conshohocken, PA, Wallcoverings in roll form – Specification for wallcoverings for
2009 subsequent decoration
BNB EN 235:2001
Lifetimes of components for life cycle analyses according to the Wallcoverings - Vocabulary and Symbols.
Bewertungssystem Nachhaltiges Bauen, 2011.
EN 259-1:2001
CDPH/EHLB Wallcoverings in roll form - Heavy duty wallcoverings - Part 1:
Standard method for measuring and evaluating chemical Specifications.
emissions from indoor sources using environmental chambers,
Version 1.1 EN ISO 105-B02
Textiles - Tests for colour fastness - Part B02: Colour fastness
CPR to artificial light: Xenon arc fading lamp test (ISO 105-
Construction Product Regulation EU B02:2014).
EN 12149:1997
Wallcoverings in roll form - Determination of migration of heavy EN ISO 14025:2006
metals and certain other elements, of vinyl chloride monomer Environmental labels and declarations — Type III
and of formaldehyde release. environmental declarations — Principles and procedures; 2009-
8 Environmental Product Declaration - IGI - The Global Wallcoverings Association - Wallcoverings on cellulose fibre base
11.
WA-101
EN ISO 14044:2006 WA Quality Standard for Polymer Coated Fabric Wallcovering
Environmental management - Life cycle assessment -
Requirements and guidelines (ISO 14044:2006).
Further documentation
EN ISO 16000:2006
Indoor air - Part 3: Determination of formaldehyde and other Ecoinvent
carbonyl compounds in indoor air and test chamber air - Active Database for Life Cycle Assessment, version 3.6. Swiss Center
sampling method. for Life Cycle Inventories, St. Gallen, 2023.
Indoor air - Part 6: Determination of volatile organic compounds
in indoor and test chamber air by active sampling on Tenax European Commission
TA® sorbent, thermal desorption and gas chromatography List of substances banned for use in cosmetic products. CMR
using MS or MS-FID. substances of category 1A, 1B or 2 under Commission
Indoor air - Part 9: Determination of the emission of volatile Regulation (EC) No 790/2009. 01/12/2010. Updated
organic compounds from building products and furnishing - 01/07/2015.
Emission test chamber method.
Indoor air - Part 11: Determination of the emission of volatile European Parliament
organic compounds from building products and furnishing - Regulation (EU) no 528/2012 of the European Parliament and
Sampling, storage of samples and preparation of test of the council of 22 may 2012 concerning the making available
specimens. on the market and use of biocidal products.
ISO 14001:2015 European Waste Catalogue (EWC)
Environmental management systems - Requirements with European Waste Catalogue / Ordinance on European List of
guidance for use. Wastes
EN 15804 EU-JRC
EN 15804:2012+A2:2019+AC:2021, Sustainability of EN 15804 reference package. Flows, Methods,
construction works — Environmental Product Declarations — Characterisation Factors, Unit Groups and Flow Properties
Core rules for the product category of construction products. based on EF Reference Package 3.0.
ISO 50001:2011 German AgBB
Energy management systems - Requirements with guidance for Committee for health-related evaluation of building products.
use. Umweltbundesamt Deutschlands.
SVHC Institut Bauen und Umwelt e. V.
Candidate List of substances of very high concern for Product Category Rules for Building-Related Products and
Authorisation (SVHC) Published in accordance with Article Services – PCR-A: Part A+A2: Calculation Rules for the Life
59(10) of the REACH Regulation. European chemicals agency Cycle Assessment and Requirements on the Project Report
(ECHA). according to EN 15804+A2:2019, version: 1.3 from 31/08/2022
RAL-GZ 479 Institut Bauen und Umwelt e. V.
Wallpapers - Quality assurance PCR Guidance-Texts for Building-Related Products and
Services - Part B: Requirements on the EPD for Wallcoverings.
Regulation (EU) No 305/2011 Version: 8 from 01/08/2021.
of the European Parliament and of the Council of 9 March 2011
laying down harmonised conditions for the marketing of LCA for Experts (GaBi)
construction products and repealing Council Directive LCA for Experts 10.7.0.183: Software System and Database for
89/106/EEC Text with EEA relevance. Current consolidated Life Cycle Engineering. 1992-2023. Sphera Solutions GmbH.
version: 16/07/2021
9 Environmental Product Declaration - IGI - The Global Wallcoverings Association - Wallcoverings on cellulose fibre base
Publisher
Institut Bauen und Umwelt e.V. +49 (0)30 3087748- 0
Hegelplatz 1 info@ibu-epd.com
10117 Berlin www.ibu-epd.com
Germany
Programme holder
Institut Bauen und Umwelt e.V. +49 (0)30 3087748- 0
Hegelplatz 1 info@ibu-epd.com
10117 Berlin www.ibu-epd.com
Germany
Author of the Life Cycle Assessment
brands & values GmbH +49 421 70 90 84 33
Altenwall 14 info@brandsandvalues.com
28195 Bremen www.brandsandvalues.com
Germany
Owner of the Declaration
IGI - The Global Wallcoverings Association +32 (0) 2 720 00 09
Chaussée de Louvain 426 info@igiwallcoverings.org
1380 LASNE www.igiwallcoverings.org
Belgium
10 Environmental Product Declaration - IGI - The Global Wallcoverings Association - Wallcoverings on cellulose fibre base
