ver1 2015
ENVIRONMENTAL PRODUCT DECLARATION
in accordance with ISO 14025, ISO 21930 and EN 15804
Owner of the declaration: Saint-Gobain Byggevarer as
Program operator: The Norwegian EPD Foundation
Publisher: The Norwegian EPD Foundation
Declaration number: NEPD-3579-2171-EN
Registration number: NEPD-3579-2171-EN
ECO Platform reference number: -
Issue date: 20.06.2022
Valid to: 20.06.2027
weber Drensmørtel / BETO Natursette-D
Saint-Gobain Byggevarer as
www.epd-norge.no
NEPD-3579-2171-EN weber Drensmørtel / BETO Natursette-D 1 / 8
General information
Product: Owner of the declaration:
weber Drensmørtel / BETO Natursette-D
Saint-Gobain Byggevarer as
Contact person: Line Holaker
Phone: +47 41 63 50 46
e-mail: info(at)weber-norge.no
Program operator: Manufacturer:
Saint-Gobain Byggevarer as
The Norwegian EPD Foundation
Pb. 5250 Majorstuen, 0303 Oslo
Phone: +47 23 08 80 00
e-mail: post@epd-norge.no
Declaration number: Place of production:
Saint-Gobain Byggevarer as
NEPD-3579-2171-EN P.O. Box 216 Alnabru 0614 Oslo, Norway
Norway
ECO Platform reference number: Management system:
ISO 9001, ISO 14001
This declaration is based on Product Category Rules: Organisation no:
940 198 178
CEN Standard EN 15804:2012+A1:2013 serves as core PCR.
NPCR 009:2018 Part B for Technical - Chemical products in the building and
construction industry
Statement of liability: Issue date: 20.06.2022
The owner of the declaration shall be liable for the underlying information and
evidence. EPD Norway shall not be liable with respect to manufacturer Valid to: 20.06.2027
information, life cycle assessment data and evidences.
Declared unit: Year of study:
1 kg weber Drensmørtel / BETO Natursette-D 2021
Declared unit with option: Comparability:
EPD of construction products may not be comparable if they not comply with EN
A1,A2,A3,A4
15804 and seen in a building context.
Functional unit: Development and verification of EPD:
The declaration has been developed and verified using EPD tool lca.tools
ver EPD2020.11, developed by LCA.no AS. The EPD tool is integrated into
the company's environmental management system, and has been
approved by EPD-Norway
General information on verification of EPD from EPD tools:
Independent verification of data, other environmental information and Developer of EPD:
the declaration according to ISO 14025:2010, § 8.1.3 and § 8.1.4. Individual
third party verification of each EPD is not required when the EPD tool is i) Line Holaker
integrated into the company's environmental management system, ii) the
procedures for use of the EPD tool are approved by EPDNorway, and iii) Reviewer of company-specific input data and EPD:
the proccess is reviewed annualy. See Appendix G of EPD-Norway's
General Programme Instructions for further information on EPD tools. Helene Løvkvist Andersen
Verification of EPD tool: Approved:
Independent third party verification of the EPD tool, background data
Sign
and test-EPD in accordance with EPDNorway's procedures and guidelines
for verification and approval of EPD tools.
Anne Rønning, Norsus AS
(no signature required) Håkon Hauan, CEO EPD-Norge
NEPD-3579-2171-EN weber Drensmørtel / BETO Natursette-D 2 / 8
Product
Product description: Technical data:
Weber Drensmørtel / BETO Natursette-D is a mortar and masonry for Compressive strength: 9 MPa after 1 day and 40 MPa after 28 days.
outdoor areas and natural stone settlements. The composition of the Flexural strength: 8 MPa after 28 days.
mass gives a very good drainage effect in the tempered mortar. This will For further information, see www.weber-norge.no and www.betomur.no
allow drainage of surface water and water in the construction and that
Market:
the mortar provides greater safety against deposits in natural stone
coatings. The product can be used for traffic areas.
Norway
Product specification
Reference service life, product
The composition of the product is described in the following table: The reference service life of the product is similar to the service life of the
construction or building.
Materials %
Binder 10-30 Reference service life, building
Aggregate 60-90
60 years
Additives <0,1
Packaging <0,5
LCA: Calculation rules
Declared unit: Allocation:
The allocation is made in accordance with the provisions of EN 15804.
1 kg weber Drensmørtel / BETO Natursette-D
Incoming energy and water and waste production in-house is allocated
Cut-off criteria: equally among all products through mass allocation. Effects of primary
production of recycled materials is allocated to the main product in
All major raw materials and all the essential energy is included. The
which the material was used. The recycling process and transportation of
production processes for raw materials and energy flows with very small
the material is allocated to this analysis.
amounts (less than 1%) are not included. These cut-off criteria do not
apply for hazardous materials and substances.
Machines and facilities (capital goods) required for and during
production are excluded, as is transportation of employees.
Data quality:
Specific data for the product composition are provided by the manufacturer. They represent the production of the declared product and were collected for
EPD development in the year of study. Background data is based on registered EPDs according to EN 15804, Ostfold Research databases, ecoinvent and other
LCA databases. The data quality of the raw materials in A1 is presented in the table below.
Plant manufacturing data is collected from previous year. The calculations are based on production in Trondheim, and delivery in 1000 kg big bags.
Transportation used in A4 is 500 km.
Materials Source Data quality Year
Aggregate Østfoldforskning Database 2016
Packaging ecoinvent 3.4 Database 2017
Cement NEPD-2274-1028-NO EPD 2020
NEPD-3579-2171-EN weber Drensmørtel / BETO Natursette-D 3 / 8
System boundary:
All processes from raw material extraction to product transport to the construction site are included in the analysis (A1-A4).
The flow chart below illustrates the system boundaries for the A1 to A3 part of the analysis. Transportation from production plant to Oslo is included in A4.
Additional technical information:
Ca. 2,5 kg/m2 (powder) pr. mm layer thickness.
100 mm thickness: ca 250 kg/m2.
Cured material is inactive and not classified as hazardous waste and may be disposed as construction waste to disposal or recycling. The packaging properly
emptied is not classified as hazardous waste.
NEPD-3579-2171-EN weber Drensmørtel / BETO Natursette-D 4 / 8
LCA: Scenarios and additional technical information
The following information describe the scenarios in the different modules of the EPD.
Transport from production place to user (A4)
Capacity utilisation Fuel/Energy
Type Type of vehicle Distance km Unit Value (l/t)
(incl. return) % consumption
Truck 55,0 % Truck, lorry over 32 tonnes, EURO 6 500 0,022606 l/tkm 11,30
Railway l/tkm
Boat l/tkm
Other Transportation l/tkm
NEPD-3579-2171-EN weber Drensmørtel / BETO Natursette-D 5 / 8
LCA: Results
The LCA results are presented below for the declared unit defined on page 2 of the EPD document.
System boundaries (X=included, MND=module not declared, MNR=module not relevant)
Construction Beyond the
Product stage installation User stage End of life stage . system
stage bondaries
A1 A2 A3 A4 A5 B1 B2 B3 B4 B5 B6 B7 C1 C2 C3 C4 . D
X X X X MND MND MND MND MND MND MND MND MND MND MND MND . MND
Environmental impact
Parameter Unit A1 A2 A3 A4
GWP kg CO 2 -eq 1,68E-01 7,61E-03 3,45E-02 4,14E-02
ODP kg CFC11 -eq 2,50E-09 1,46E-09 3,86E-09 8,50E-09
POCP kg C 2H 4-eq 2,17E-05 1,51E-06 9,44E-06 6,47E-06
AP kg SO 2 -eq 7,52E-05 4,78E-05 7,03E-05 1,07E-04
EP kg PO 3- -eq 9,22E-05 9,20E-06 2,16E-05 1,47E-05
4
ADPM kg Sb -eq 5,83E-08 7,37E-09 2,46E-08 9,85E-08
ADPE MJ 5,51E-01 1,14E-01 3,21E-01 6,79E-01
GWP Global warming potential; ODP Depletion potential of the stratospheric ozone layer; POCP Formation potential of tropospheric photochemical oxidants;
AP Acidification potential of land and water; EP Eutrophication potential; ADPM Abiotic depletion potential for non fossil resources; ADPE Abiotic depletion
potential for fossil resources
Reading example: 9,0 E-03 = 9,0*10-3 = 0,009
*INA Indicator Not Assessed
Remarks to environmental impacts
No environmental impacts from the product.
waR slairetam tropsnarT gnirutcafunaM tropsnarT ylbmessA esU ecnanetniaM riapeR tnemecalpeR tnemhsibrufeR lanoitarepO ygrene esu lanoitarepO esu
retaw
-eD noitcurtsnoc noitilomed tropsnarT etsaW gnissecorp lasopsiD -yrevoceR-esueR -gnilcyceR laitnetop
NEPD-3579-2171-EN weber Drensmørtel / BETO Natursette-D 6 / 8
Resource use
Parameter Unit A1 A2 A3 A4
RPEE MJ 1,53E-01 1,18E-03 1,23E-01 1,24E-02
RPEM MJ 0,00E+00 0,00E+00 0,00E+00 0,00E+00
TPE MJ 1,53E-01 1,18E-03 1,23E-01 1,24E-02
NRPE MJ 5,79E-01 1,16E-01 3,35E-01 7,01E-01
NRPM MJ 7,26E-02 0,00E+00 0,00E+00 0,00E+00
TRPE MJ 6,51E-01 1,16E-01 3,35E-01 7,01E-01
SM kg 7,26E-02 0,00E+00 0,00E+00 0,00E+00
RSF MJ 2,32E-01 0,00E+00 2,01E-05 0,00E+00
NRSF MJ 2,94E-01 0,00E+00 0,00E+00 0,00E+00
W m3 1,14E-03 1,66E-05 4,88E-05 1,66E-04
RPEE Renewable primary energy resources used as energy carrier; RPEM Renewable primary energy resources used as raw materials; TPE Total use of renewable
primary energy resources; NRPE Non renewable primary energy resources used as energy carrier; NRPM Non renewable primary energy resources used as
materials; TRPE Total use of non renewable primary energy resources; SM Use of secondary materials; RSF Use of renewable secondary fuels; NRSF Use of non
renewable secondary fuels; W Use of net fresh water
Reading example: 9,0 E-03 = 9,0*10-3 = 0,009
*INA Indicator Not Assessed
End of life - Waste
Parameter Unit A1 A2 A3 A4
HW kg 5,25E-07 5,36E-08 8,32E-05 3,74E-07
NHW kg 2,06E-02 4,13E-03 2,31E-02 6,40E-02
RW kg INA* INA* INA* INA*
HW Hazardous waste disposed; NHW Non hazardous waste disposed; RW Radioactive waste disposed
Reading example: 9,0 E-03 = 9,0*10-3 = 0,009
*INA Indicator Not Assessed
End of life - Output flow
Parameter Unit A1 A2 A3 A4
CR kg 0,00E+00 0,00E+00 0,00E+00 0,00E+00
MR kg 0,00E+00 0,00E+00 1,86E-04 0,00E+00
MER kg 0,00E+00 0,00E+00 6,90E-04 0,00E+00
EEE MJ INA* INA* INA* INA*
ETE MJ INA* INA* INA* INA*
CR Components for reuse; MR Materials for recycling; MER Materials for energy recovery; EEE Exported electric energy; ETE Exported thermal energy
Reading example: 9,0 E-03 = 9,0*10-3 = 0,009
*INA Indicator Not Assessed
NEPD-3579-2171-EN weber Drensmørtel / BETO Natursette-D 7 / 8
Additional Norwegian requirements
Greenhouse gas emissions from the use of electricity in the manufacturing phase
National production mix from import, low voltage (production of transmission lines, in addition to direct emissions and losses in grid) of applied electricity for
the manufacturing process (A3).
Electricity mix Data source Amount Unit
El-mix, Norway (kWh) ecoinvent 3.4 31,04 g CO2-ekv/kWh
Dangerous substances
The product contains no substances given by the REACH Candidate list or the Norwegian priority list. The product is classified as hazardous waste
(Avfallsforskriften, Annex III), see table.
Name CASNo Amount
Portland Cement 65997-15-1 10-30%
Indoor environment
The product has no impact on the indoor environment.
Bibliography
ISO 14025:2010 Environmental labels and declarations - Type III environmental declarations - Principles and procedures.
ISO 14044:2006 Environmental management - Life cycle assessment - Requirements and guidelines.
EN 15804:2012+A1:2013 Environmental product declaration - Core rules for the product category of construction products.
ISO 21930:2017 Sustainability in buildings and civil engineering works. Core rules for environmental product declarations of construction products.
ecoinvent v3, Allocation, cut-off by classification, Swiss Centre of Life Cycle Inventories.
Iversen et al., (2018) eEPD v3.0 - Background information for EPD generator system, LCA.no report number 04.18
Iversen et al., (2019) EPD generator for Saint-Gobain Weber and Scanspac - Background information and LCA data, LCA.no report number 05.18
NPCR Part A: Construction products and services. Ver. 1.0. April 2017, EPD-Norge.
NPCR 009 Part B for technical-chemical products. Ver. 1.0 June 2018, EPD-Norge.
Program operator and publisher Phone: +47 23 08 80 00
The Norwegian EPD Foundation e-mail: post@epd-norge.no
Post Box 5250 Majorstuen, 0303 Oslo,Norway web: www.epd-norge.no
Owner of the declaration Phone: +47 41 63 50 46
Saint-Gobain Byggevarer as e-mail: info(at)weber-norge.no
P.O. Box 216 Alnabru 0614 Oslo, Norway web: www.weber-norge.no
Author of the Life Cycle Assessment Phone: +47 916 50 916
LCA.no AS e-mail: post@lca.no
Dokka 6B 1671 Kråkerøy web: www.lca.no
Developer of EPD generator Phone: +47 916 50 916
LCA.no AS e-mail: post@lca.no
Dokka 1C,1671 Kråkerøy web: www.lca.no
NEPD-3579-2171-EN weber Drensmørtel / BETO Natursette-D 8 / 8
