ver1 2015
ENVIRONMENTAL PRODUCT DECLARATION
in accordance with ISO 14025, ISO 21930 and EN 15804
Owner of the declaration: Saint-Gobain Sweden AB, Weber
Program operator: The Norwegian EPD Foundation
The Norwegian EPD Foundation
Publisher:
Declaration number: NEPD-2024-895-EN
Registration number: NEPD-2024-895-EN
ECO Platform reference number: -
Issue date: 23.01.2020
Valid to: 23.01.2025
webertherm 261 putsbruk EF
Saint-Gobain Sweden AB, Weber
www.epd-norge.no
General information
Product: Owner of the declaration:
webertherm 261 putsbruk EF Saint-Gobain Sweden AB, Weber
Contact person: Anders Anderberg
Phone: +46 8 625 6105
e-mail: anders.anderberg@weber.se
Program operator: Manufacturer:
The Norwegian EPD Foundation Saint-Gobain Sweden AB, Weber
Pb. 5250 Majorstuen, 0303 Oslo
Phone: +47 97722020
e-mail: post@epd-norge.no
Declaration number: Place of production:
NEPD-2024-895-EN Saint-Gobain Sweden AB, Weber, Riksten
ECO Platform reference number: Management system:
ISO 9001, ISO 14001
This declaration is based on Product Category Rules: Organisation no:
CEN Standard EN 15804:2012+A1:2013 serves as core PCR. SE-556241-2592
Requirements on the EPD for Mineral factory-made mortar.
Statement of liability: Issue date: 23.01.2020
The owner of the declaration shall be liable for the underlying
information and evidence. EPD Norway shall not be liable with Valid to: 23.01.2025
respect to manufacturer information, life cycle assessment data and
evidences.
Declared unit: Year of study:
1 kg webertherm 261 putsbruk EF 2018
Declared unit with option: Comparability:
EPD of construction products may not be comparable if they not
A1,A2,A3,A4
comply with EN 15804 and seen in a building context.
Functional unit: Author of the Life Cycle Assessment:
The declaration is developed using eEPD v3.0 from LCA.no
Approval:
Company specific data are:
Collected/registered by: Charlotte Karlsson
Internal verification by: Helene Wallgren
Verification: Approved:
Independent verification of data, other environmental information and
the declaration according to ISO14025:2010, § 8.1.3 and § 8.1.4
External
Third party verifier:
Sign Sign
Senior Research Scientist, Anne Rønning
(Independent verifier approved by EPD Norway)
Product
Product description: Technical data:
webertherm 261 putsbruk EF is a factory-made fiber-reinforced dry mortar webertherm 261 putsbruk EF is tested and approved according to EN 998-
based on lime and cement with natural sand as aggregates. When mixed 1 and ETA SP 105 Fire.
with water, it is a ready-to-use render for indor and outdoor use.
webertherm 261 putsbruk EF is a hydrofobic render specially designed for Mortar category: CS III.
use in Serpomin EF facade systems and Serpovent G2. webertherm 261
putsbruk EF can also be used on both Exclay,bricks and Concrete as well For further information, see www.se.weber/
as previously renderd facades. webertherm 261 putsbruk EF is applied in
Market:
two layers, the first layer (> 6mm), and the second layer around 2-3 mm.
The render is sprayable and pumpable in a 60m hose. Sweden and Denmark
Reference service life, product
webertherm 261 putsbruk EF can be delivered in closed silos of 10 tons
with a flow mixer to avoid dust. The reference service life of the product is similar to the service life of the
building.
Product specification
Reference service life, building
50 years.
Materials %
Binder 10-30
Aggregate 60-90
Filler 5-10
Additives <5
Packaging <0,2
LCA: Calculation rules
Declared unit: Allocation:
The allocation is made in accordance with the provisions of EN 15804.
1 kg webertherm 261 putsbruk EF
Incoming energy and water and waste production in-house is allocated
Cut-off criteria: equally among all products through mass allocation. Effects of primary
All major raw materials and all the essential energy is included. The production of recycled materials is allocated to the main product in which
production processes for raw materials and energy flows with very small the material was used. The recycling process and transportation of the
amounts (less than 1%) are not included. These cut-off criteria do not material is allocated to this analysis.
apply for hazardous materials and substances.
Data quality:
Specific data for the product composition are provided by the manufacturer. They represent the production of the declared product and were collected
for EPD development in the year of study. Background data is based on registered EPDs according to EN 15804, Ostfold Research databases,
ecoinvent and other LCA databases. The data quality of the raw materials in A1 is presented in the table below.
Materials Source Data quality Year
Cement Supplier EPD 2014
Additives ecoinvent 3.4 Database 2017
Aggregate ecoinvent 3.4 Database 2017
Filler ecoinvent 3.4 Database 2017
Packaging ecoinvent 3.4 Database 2017
Packaging Modified ecoinvent 3.4 Database 2017
SC 99 Owner of EPD Database
SC 354 Owner of EPD Database 2018
SC 425 Owner of EPD Database 2019
System boundary:
"All processes from raw material extraction to product from the factory gate are included in the analysis (A1-A3). In addition, transportation to a central
warehouse placed in accordance with guidelines issued by the EPD Norway (A4) is included.
The flow chart below illustrates the system boundaries for the A1 to A3 part of the analysis."
Additional technical information:
webertherm 261 putsbruk EF is a render in the ventilated Serpovent G2 , Serpovent G2 has been verified for fire according to SP 105 Fire.
The remaining powder is classified as hazardous waste. Cured material is inactive and not classified as hazardous waste and may be disposed as
construction waste to disposal or recycling.
The packaging properly emptied is not classified as hazardous waste.
LCA: Scenarios and additional technical information
The following information describe the scenarios in the different modules of the EPD.
Transport from production place to user (A4)
Capacity
Fuel/Energy
Type utilisation (incl. Type of vehicle Distance km Unit Value (l/t)
consumption
return) %
Truck, lorry over
Truck 55,0 % 32 tonnes, EURO 152 0,022823 l/tkm 3,47
5
Railway l/tkm
Boat l/tkm
Other Transportation l/tkm
LCA: Results
System boundaries (X=included, MND=module not declared, MNR=module not relevant)
Construction Beyond the
Product stage installation User stage End of life stage . system
stage bondaries
A1 A2 A3 A4 A5 B1 B2 B3 B4 B5 B6 B7 C1 C2 C3 C4 . D
X X X X MND MND MND MND MND MND MND MND MND MND MND MND . MND
Environmental impact
Parameter Unit A1 A2 A3 A4
GWP kg CO 2 -eq 2,05E-01 1,48E-02 2,02E-02 1,33E-02
ODP kg CFC11 -eq 6,37E-09 2,27E-09 4,16E-09 2,58E-09
POCP kg C 2H 4-eq 4,32E-05 2,43E-06 6,18E-06 2,14E-06
AP kg SO 2 -eq 4,66E-04 5,00E-05 1,11E-04 4,31E-05
EP kg PO3- -eq 1,33E-04 8,52E-06 2,45E-05 7,23E-06
4
ADPM kg Sb -eq 5,45E-07 4,36E-08 1,97E-08 2,99E-08
ADPE MJ 2,58E+00 2,24E-01 3,23E-01 2,08E-01
GWP Global warming potential; ODP Depletion potential of the stratospheric ozone layer; POCP Formation potential of tropospheric photochemical
oxidants; AP Acidification potential of land and water; EP Eutrophication potential; ADPM Abiotic depletion potential for non fossil resources; ADPE
Abiotic depletion potential for fossil resources
Reading example: 9,0 E-03 = 9,0*10-3 = 0,009
*INA Indicator Not Assessed
waR slairetam tropsnarT
gnirutcafunaM
tropsnarT ylbmessA esU ecnanetniaM riapeR tnemecalpeR
tnemhsibrufeR
lanoitarepO ygrene esu lanoitarepO esu retaw -eD noitcurtsnoc noitilomed tropsnarT etsaW gnissecorp lasopsiD
-yrevoceR-esueR
-gnilcyceR laitnetop
NEPD-2024-895-EN webertherm 261 putsbruk EF 1 / 8
Resource use
Parameter Unit A1 A2 A3 A4
RPEE MJ 3,52E-01 3,32E-03 2,63E-01 3,76E-03
RPEM MJ 1,02E-01 0,00E+00 0,00E+00 0,00E+00
TPE MJ 4,54E-01 3,32E-03 2,63E-01 3,76E-03
NRPE MJ 2,85E+00 2,30E-01 3,25E-01 2,14E-01
NRPM MJ 9,54E-02 0,00E+00 0,00E+00 0,00E+00
TRPE MJ 2,95E+00 2,30E-01 3,25E-01 2,14E-01
SM kg 8,71E-04 0,00E+00 0,00E+00 0,00E+00
RSF MJ 7,58E-02 0,00E+00 0,00E+00 0,00E+00
NRSF MJ 1,04E-01 0,00E+00 0,00E+00 0,00E+00
W m3 2,72E-03 4,66E-05 4,04E-05 5,05E-05
RPEE Renewable primary energy resources used as energy carrier; RPEM Renewable primary energy resources used as raw materials; TPE Total use
of renewable primary energy resources; NRPE Non renewable primary energy resources used as energy carrier; NRPM Non renewable primary energy
resources used as materials; TRPE Total use of non renewable primary energy resources; SM Use of secondary materials; RSF Use of renewable
secondary fuels; NRSF Use of non renewable secondary fuels; W Use of net fresh water
Reading example: 9,0 E-03 = 9,0*10-3 = 0,009
*INA Indicator Not Assessed
End of life - Waste
Parameter Unit A1 A2 A3 A4
HW kg 1,76E-06 1,37E-07 2,28E-05 1,14E-07
NHW kg 1,99E-02 1,31E-02 6,81E-02 1,95E-02
RW kg INA* INA* INA* INA*
HW Hazardous waste disposed; NHW Non hazardous waste disposed; RW Radioactive waste disposed
Reading example: 9,0 E-03 = 9,0*10-3 = 0,009
*INA Indicator Not Assessed
End of life - Output flow
Parameter Unit A1 A2 A3 A4
CR kg 0,00E+00 0,00E+00 0,00E+00 0,00E+00
MR kg 7,84E-08 0,00E+00 3,68E-04 0,00E+00
MER kg 3,21E-06 0,00E+00 1,55E-03 0,00E+00
EEE MJ INA* INA* INA* INA*
ETE MJ INA* INA* INA* INA*
CR Components for reuse; MR Materials for recycling; MER Materials for energy recovery; EEE Exported electric energy; ETE Exported thermal
energy
Reading example: 9,0 E-03 = 9,0*10-3 = 0,009
*INA Indicator Not Assessed
Additional Norwegian requirements
Greenhouse gas emissions from the use of electricity in the manufacturing phase
National production mix from import, low voltage (production of transmission lines, in addition to direct emissions and losses in grid) of applied
electricity for the manufacturing process (A3).
Electricity mix Data source Amount Unit
Renewable electricity with Guarantee of Origin from LOS (kWh) Modified ecoinvent 3.4 60,20 g CO2-ekv/kWh
Dangerous substances
The product contains no substances given by the REACH Candidate list or the Norwegian priority list. The product is classified as hazardous waste
(Avfallsforskriften, Annex III), see table.
Name CASNo Amount
Portand Cement 65997-15-1 10-20%
Indoor environment
The product has no impact on the indoor environment.
Bibliography
ISO 14025:2010 Environmental labels and declarations - Type III environmental declarations - Principles and procedures.
ISO 14044:2006 Environmental management - Life cycle assessment - Requirements and guidelines.
EN 15804:2012+A1:2013 Environmental product declaration - Core rules for the product category of construction products.
ISO 21930:2017 Sustainability in buildings and civil engineering works. Core rules for environmental product declarations of construction products.
ecoinvent v3, Allocation, cut-off by classification, Swiss Centre of Life Cycle Inventories.
Iversen et al., (2018) eEPD v3.0 - Background information for EPD generator system, LCA.no report number 04.18
Iversen et al., (2019) EPD generator for Saint-Gobain Weber and Scanspac - Background information and LCA data, LCA.no report number 05.18
NPCR Part A: Construction products and services. Ver. 1.0. April 2017, EPD-Norge.
NPCR 009 Part B for technical-chemical products. Ver. 1.0 June 2018, EPD-Norge.
Product Category Rules for Environmental Product Declarations: Institut Bauen und Umwelt e.V. (IBU): Requirements on the EPD for Mineral
factorymade
mortar.
Program operator and publisher Phone: +47 97722020
The Norwegian EPD Foundation
Post Box 5250 Majorstuen, 0303 Oslo e-mail: post@epd-norge.no
0303 Oslo Norway web: www.epd-norge.no
Owner of the declaration Phone: +46 8 625 6105
Saint-Gobain Sweden AB, Weber Fax:
Box 415 e-mail: anders.anderberg@weber.se
SE-19162 Sollentuna web: www.weber.se
Author of the Life Cycle Assessment Phone: +47 916 50 916
LCA.no AS Fax:
Dokka 1C e-mail: post@lca.no
1671 Kråkerøy web: www.lca.no
Developer of EPD generator Phone: +47 916 50 916
LCA.no AS
Dokka 1C e-mail: post@lca.no
1671 Kråkerøy web: www.lca.no
ver1 2015
ENVIRONMENTAL PRODUCT DECLARATION
in accordance with ISO 14025, ISO 21930 and EN 15804
Owner of the declaration: Saint-Gobain Sweden AB, Weber
Program operator: The Norwegian EPD Foundation
The Norwegian EPD Foundation
Publisher:
Declaration number: NEPD-2024-895-EN
Registration number: NEPD-2024-895-EN
ECO Platform reference number: -
Issue date: 23.01.2020
Valid to: 23.01.2025
webertherm 261 putsbruk EF
Saint-Gobain Sweden AB, Weber
www.epd-norge.no
General information
Product: Owner of the declaration:
webertherm 261 putsbruk EF Saint-Gobain Sweden AB, Weber
Contact person: Anders Anderberg
Phone: +46 8 625 6105
e-mail: anders.anderberg@weber.se
Program operator: Manufacturer:
The Norwegian EPD Foundation Saint-Gobain Sweden AB, Weber
Pb. 5250 Majorstuen, 0303 Oslo
Phone: +47 97722020
e-mail: post@epd-norge.no
Declaration number: Place of production:
NEPD-2024-895-EN Saint-Gobain Sweden AB, Weber, Riksten
ECO Platform reference number: Management system:
ISO 9001, ISO 14001
This declaration is based on Product Category Rules: Organisation no:
CEN Standard EN 15804:2012+A1:2013 serves as core PCR. SE-556241-2592
Requirements on the EPD for Mineral factory-made mortar.
Statement of liability: Issue date: 23.01.2020
The owner of the declaration shall be liable for the underlying
information and evidence. EPD Norway shall not be liable with Valid to: 23.01.2025
respect to manufacturer information, life cycle assessment data and
evidences.
Declared unit: Year of study:
1 kg webertherm 261 putsbruk EF 2018
Declared unit with option: Comparability:
EPD of construction products may not be comparable if they not
A1,A2,A3,A4
comply with EN 15804 and seen in a building context.
Functional unit: Author of the Life Cycle Assessment:
The declaration is developed using eEPD v3.0 from LCA.no
Approval:
Company specific data are:
Collected/registered by: Charlotte Karlsson
Internal verification by: Helene Wallgren
Verification: Approved:
Independent verification of data, other environmental information and
the declaration according to ISO14025:2010, § 8.1.3 and § 8.1.4
External
Third party verifier:
Sign Sign
Senior Research Scientist, Anne Rønning
(Independent verifier approved by EPD Norway)
Product
Product description: Technical data:
webertherm 261 putsbruk EF is a factory-made fiber-reinforced dry mortar webertherm 261 putsbruk EF is tested and approved according to EN 998-
based on lime and cement with natural sand as aggregates. When mixed 1 and ETA SP 105 Fire.
with water, it is a ready-to-use render for indor and outdoor use.
webertherm 261 putsbruk EF is a hydrofobic render specially designed for Mortar category: CS III.
use in Serpomin EF facade systems and Serpovent G2. webertherm 261
putsbruk EF can also be used on both Exclay,bricks and Concrete as well For further information, see www.se.weber/
as previously renderd facades. webertherm 261 putsbruk EF is applied in
Market:
two layers, the first layer (> 6mm), and the second layer around 2-3 mm.
The render is sprayable and pumpable in a 60m hose. Sweden and Denmark
Reference service life, product
webertherm 261 putsbruk EF can be delivered in closed silos of 10 tons
with a flow mixer to avoid dust. The reference service life of the product is similar to the service life of the
building.
Product specification
Reference service life, building
50 years.
Materials %
Binder 10-30
Aggregate 60-90
Filler 5-10
Additives <5
Packaging <0,2
LCA: Calculation rules
Declared unit: Allocation:
The allocation is made in accordance with the provisions of EN 15804.
1 kg webertherm 261 putsbruk EF
Incoming energy and water and waste production in-house is allocated
Cut-off criteria: equally among all products through mass allocation. Effects of primary
All major raw materials and all the essential energy is included. The production of recycled materials is allocated to the main product in which
production processes for raw materials and energy flows with very small the material was used. The recycling process and transportation of the
amounts (less than 1%) are not included. These cut-off criteria do not material is allocated to this analysis.
apply for hazardous materials and substances.
Data quality:
Specific data for the product composition are provided by the manufacturer. They represent the production of the declared product and were collected
for EPD development in the year of study. Background data is based on registered EPDs according to EN 15804, Ostfold Research databases,
ecoinvent and other LCA databases. The data quality of the raw materials in A1 is presented in the table below.
Materials Source Data quality Year
Cement Supplier EPD 2014
Additives ecoinvent 3.4 Database 2017
Aggregate ecoinvent 3.4 Database 2017
Filler ecoinvent 3.4 Database 2017
Packaging ecoinvent 3.4 Database 2017
Packaging Modified ecoinvent 3.4 Database 2017
SC 99 Owner of EPD Database
SC 354 Owner of EPD Database 2018
SC 425 Owner of EPD Database 2019
System boundary:
"All processes from raw material extraction to product from the factory gate are included in the analysis (A1-A3). In addition, transportation to a central
warehouse placed in accordance with guidelines issued by the EPD Norway (A4) is included.
The flow chart below illustrates the system boundaries for the A1 to A3 part of the analysis."
Additional technical information:
webertherm 261 putsbruk EF is a render in the ventilated Serpovent G2 , Serpovent G2 has been verified for fire according to SP 105 Fire.
The remaining powder is classified as hazardous waste. Cured material is inactive and not classified as hazardous waste and may be disposed as
construction waste to disposal or recycling.
The packaging properly emptied is not classified as hazardous waste.
LCA: Scenarios and additional technical information
The following information describe the scenarios in the different modules of the EPD.
Transport from production place to user (A4)
Capacity
Fuel/Energy
Type utilisation (incl. Type of vehicle Distance km Unit Value (l/t)
consumption
return) %
Truck, lorry over
Truck 55,0 % 32 tonnes, EURO 152 0,022823 l/tkm 3,47
5
Railway l/tkm
Boat l/tkm
Other Transportation l/tkm
LCA: Results
System boundaries (X=included, MND=module not declared, MNR=module not relevant)
Construction Beyond the
Product stage installation User stage End of life stage . system
stage bondaries
A1 A2 A3 A4 A5 B1 B2 B3 B4 B5 B6 B7 C1 C2 C3 C4 . D
X X X X MND MND MND MND MND MND MND MND MND MND MND MND . MND
Environmental impact
Parameter Unit A1 A2 A3 A4
GWP kg CO 2 -eq 2,05E-01 1,48E-02 2,02E-02 1,33E-02
ODP kg CFC11 -eq 6,37E-09 2,27E-09 4,16E-09 2,58E-09
POCP kg C 2H 4-eq 4,32E-05 2,43E-06 6,18E-06 2,14E-06
AP kg SO 2 -eq 4,66E-04 5,00E-05 1,11E-04 4,31E-05
EP kg PO3- -eq 1,33E-04 8,52E-06 2,45E-05 7,23E-06
4
ADPM kg Sb -eq 5,45E-07 4,36E-08 1,97E-08 2,99E-08
ADPE MJ 2,58E+00 2,24E-01 3,23E-01 2,08E-01
GWP Global warming potential; ODP Depletion potential of the stratospheric ozone layer; POCP Formation potential of tropospheric photochemical
oxidants; AP Acidification potential of land and water; EP Eutrophication potential; ADPM Abiotic depletion potential for non fossil resources; ADPE
Abiotic depletion potential for fossil resources
Reading example: 9,0 E-03 = 9,0*10-3 = 0,009
*INA Indicator Not Assessed
waR slairetam tropsnarT
gnirutcafunaM
tropsnarT ylbmessA esU ecnanetniaM riapeR tnemecalpeR
tnemhsibrufeR
lanoitarepO ygrene esu lanoitarepO esu retaw -eD noitcurtsnoc noitilomed tropsnarT etsaW gnissecorp lasopsiD
-yrevoceR-esueR
-gnilcyceR laitnetop
NEPD-2024-895-EN webertherm 261 putsbruk EF 2 / 8
Resource use
Parameter Unit A1 A2 A3 A4
RPEE MJ 3,52E-01 3,32E-03 2,63E-01 3,76E-03
RPEM MJ 1,02E-01 0,00E+00 0,00E+00 0,00E+00
TPE MJ 4,54E-01 3,32E-03 2,63E-01 3,76E-03
NRPE MJ 2,85E+00 2,30E-01 3,25E-01 2,14E-01
NRPM MJ 9,54E-02 0,00E+00 0,00E+00 0,00E+00
TRPE MJ 2,95E+00 2,30E-01 3,25E-01 2,14E-01
SM kg 8,71E-04 0,00E+00 0,00E+00 0,00E+00
RSF MJ 7,58E-02 0,00E+00 0,00E+00 0,00E+00
NRSF MJ 1,04E-01 0,00E+00 0,00E+00 0,00E+00
W m3 2,72E-03 4,66E-05 4,04E-05 5,05E-05
RPEE Renewable primary energy resources used as energy carrier; RPEM Renewable primary energy resources used as raw materials; TPE Total use
of renewable primary energy resources; NRPE Non renewable primary energy resources used as energy carrier; NRPM Non renewable primary energy
resources used as materials; TRPE Total use of non renewable primary energy resources; SM Use of secondary materials; RSF Use of renewable
secondary fuels; NRSF Use of non renewable secondary fuels; W Use of net fresh water
Reading example: 9,0 E-03 = 9,0*10-3 = 0,009
*INA Indicator Not Assessed
End of life - Waste
Parameter Unit A1 A2 A3 A4
HW kg 1,76E-06 1,37E-07 2,28E-05 1,14E-07
NHW kg 1,99E-02 1,31E-02 6,81E-02 1,95E-02
RW kg INA* INA* INA* INA*
HW Hazardous waste disposed; NHW Non hazardous waste disposed; RW Radioactive waste disposed
Reading example: 9,0 E-03 = 9,0*10-3 = 0,009
*INA Indicator Not Assessed
End of life - Output flow
Parameter Unit A1 A2 A3 A4
CR kg 0,00E+00 0,00E+00 0,00E+00 0,00E+00
MR kg 7,84E-08 0,00E+00 3,68E-04 0,00E+00
MER kg 3,21E-06 0,00E+00 1,55E-03 0,00E+00
EEE MJ INA* INA* INA* INA*
ETE MJ INA* INA* INA* INA*
CR Components for reuse; MR Materials for recycling; MER Materials for energy recovery; EEE Exported electric energy; ETE Exported thermal
energy
Reading example: 9,0 E-03 = 9,0*10-3 = 0,009
*INA Indicator Not Assessed
Additional Norwegian requirements
Greenhouse gas emissions from the use of electricity in the manufacturing phase
National production mix from import, low voltage (production of transmission lines, in addition to direct emissions and losses in grid) of applied
electricity for the manufacturing process (A3).
Electricity mix Data source Amount Unit
Renewable electricity with Guarantee of Origin from LOS (kWh) Modified ecoinvent 3.4 60,20 g CO2-ekv/kWh
Dangerous substances
The product contains no substances given by the REACH Candidate list or the Norwegian priority list. The product is classified as hazardous waste
(Avfallsforskriften, Annex III), see table.
Name CASNo Amount
Portand Cement 65997-15-1 10-20%
Indoor environment
The product has no impact on the indoor environment.
Bibliography
ISO 14025:2010 Environmental labels and declarations - Type III environmental declarations - Principles and procedures.
ISO 14044:2006 Environmental management - Life cycle assessment - Requirements and guidelines.
EN 15804:2012+A1:2013 Environmental product declaration - Core rules for the product category of construction products.
ISO 21930:2017 Sustainability in buildings and civil engineering works. Core rules for environmental product declarations of construction products.
ecoinvent v3, Allocation, cut-off by classification, Swiss Centre of Life Cycle Inventories.
Iversen et al., (2018) eEPD v3.0 - Background information for EPD generator system, LCA.no report number 04.18
Iversen et al., (2019) EPD generator for Saint-Gobain Weber and Scanspac - Background information and LCA data, LCA.no report number 05.18
NPCR Part A: Construction products and services. Ver. 1.0. April 2017, EPD-Norge.
NPCR 009 Part B for technical-chemical products. Ver. 1.0 June 2018, EPD-Norge.
Product Category Rules for Environmental Product Declarations: Institut Bauen und Umwelt e.V. (IBU): Requirements on the EPD for Mineral
factorymade
mortar.
Program operator and publisher Phone: +47 97722020
The Norwegian EPD Foundation
Post Box 5250 Majorstuen, 0303 Oslo e-mail: post@epd-norge.no
0303 Oslo Norway web: www.epd-norge.no
Owner of the declaration Phone: +46 8 625 6105
Saint-Gobain Sweden AB, Weber Fax:
Box 415 e-mail: anders.anderberg@weber.se
SE-19162 Sollentuna web: www.weber.se
Author of the Life Cycle Assessment Phone: +47 916 50 916
LCA.no AS Fax:
Dokka 1C e-mail: post@lca.no
1671 Kråkerøy web: www.lca.no
Developer of EPD generator Phone: +47 916 50 916
LCA.no AS
Dokka 1C e-mail: post@lca.no
1671 Kråkerøy web: www.lca.no
ver1 2015
ENVIRONMENTAL PRODUCT DECLARATION
in accordance with ISO 14025, ISO 21930 and EN 15804
Owner of the declaration: Saint-Gobain Sweden AB, Weber
Program operator: The Norwegian EPD Foundation
The Norwegian EPD Foundation
Publisher:
Declaration number: NEPD-2024-895-EN
Registration number: NEPD-2024-895-EN
ECO Platform reference number: -
Issue date: 23.01.2020
Valid to: 23.01.2025
webertherm 261 putsbruk EF
Saint-Gobain Sweden AB, Weber
www.epd-norge.no
General information
Product: Owner of the declaration:
webertherm 261 putsbruk EF Saint-Gobain Sweden AB, Weber
Contact person: Anders Anderberg
Phone: +46 8 625 6105
e-mail: anders.anderberg@weber.se
Program operator: Manufacturer:
The Norwegian EPD Foundation Saint-Gobain Sweden AB, Weber
Pb. 5250 Majorstuen, 0303 Oslo
Phone: +47 97722020
e-mail: post@epd-norge.no
Declaration number: Place of production:
NEPD-2024-895-EN Saint-Gobain Sweden AB, Weber, Riksten
ECO Platform reference number: Management system:
ISO 9001, ISO 14001
This declaration is based on Product Category Rules: Organisation no:
CEN Standard EN 15804:2012+A1:2013 serves as core PCR. SE-556241-2592
Requirements on the EPD for Mineral factory-made mortar.
Statement of liability: Issue date: 23.01.2020
The owner of the declaration shall be liable for the underlying
information and evidence. EPD Norway shall not be liable with Valid to: 23.01.2025
respect to manufacturer information, life cycle assessment data and
evidences.
Declared unit: Year of study:
1 kg webertherm 261 putsbruk EF 2018
Declared unit with option: Comparability:
EPD of construction products may not be comparable if they not
A1,A2,A3,A4
comply with EN 15804 and seen in a building context.
Functional unit: Author of the Life Cycle Assessment:
The declaration is developed using eEPD v3.0 from LCA.no
Approval:
Company specific data are:
Collected/registered by: Charlotte Karlsson
Internal verification by: Helene Wallgren
Verification: Approved:
Independent verification of data, other environmental information and
the declaration according to ISO14025:2010, § 8.1.3 and § 8.1.4
External
Third party verifier:
Sign Sign
Senior Research Scientist, Anne Rønning
(Independent verifier approved by EPD Norway)
Product
Product description: Technical data:
webertherm 261 putsbruk EF is a factory-made fiber-reinforced dry mortar webertherm 261 putsbruk EF is tested and approved according to EN 998-
based on lime and cement with natural sand as aggregates. When mixed 1 and ETA SP 105 Fire.
with water, it is a ready-to-use render for indor and outdoor use.
webertherm 261 putsbruk EF is a hydrofobic render specially designed for Mortar category: CS III.
use in Serpomin EF facade systems and Serpovent G2. webertherm 261
putsbruk EF can also be used on both Exclay,bricks and Concrete as well For further information, see www.se.weber/
as previously renderd facades. webertherm 261 putsbruk EF is applied in
Market:
two layers, the first layer (> 6mm), and the second layer around 2-3 mm.
The render is sprayable and pumpable in a 60m hose. Sweden and Denmark
Reference service life, product
webertherm 261 putsbruk EF can be delivered in closed silos of 10 tons
with a flow mixer to avoid dust. The reference service life of the product is similar to the service life of the
building.
Product specification
Reference service life, building
50 years.
Materials %
Binder 10-30
Aggregate 60-90
Filler 5-10
Additives <5
Packaging <0,2
LCA: Calculation rules
Declared unit: Allocation:
The allocation is made in accordance with the provisions of EN 15804.
1 kg webertherm 261 putsbruk EF
Incoming energy and water and waste production in-house is allocated
Cut-off criteria: equally among all products through mass allocation. Effects of primary
All major raw materials and all the essential energy is included. The production of recycled materials is allocated to the main product in which
production processes for raw materials and energy flows with very small the material was used. The recycling process and transportation of the
amounts (less than 1%) are not included. These cut-off criteria do not material is allocated to this analysis.
apply for hazardous materials and substances.
Data quality:
Specific data for the product composition are provided by the manufacturer. They represent the production of the declared product and were collected
for EPD development in the year of study. Background data is based on registered EPDs according to EN 15804, Ostfold Research databases,
ecoinvent and other LCA databases. The data quality of the raw materials in A1 is presented in the table below.
Materials Source Data quality Year
Cement Supplier EPD 2014
Additives ecoinvent 3.4 Database 2017
Aggregate ecoinvent 3.4 Database 2017
Filler ecoinvent 3.4 Database 2017
Packaging ecoinvent 3.4 Database 2017
Packaging Modified ecoinvent 3.4 Database 2017
SC 99 Owner of EPD Database
SC 354 Owner of EPD Database 2018
SC 425 Owner of EPD Database 2019
System boundary:
"All processes from raw material extraction to product from the factory gate are included in the analysis (A1-A3). In addition, transportation to a central
warehouse placed in accordance with guidelines issued by the EPD Norway (A4) is included.
The flow chart below illustrates the system boundaries for the A1 to A3 part of the analysis."
Additional technical information:
webertherm 261 putsbruk EF is a render in the ventilated Serpovent G2 , Serpovent G2 has been verified for fire according to SP 105 Fire.
The remaining powder is classified as hazardous waste. Cured material is inactive and not classified as hazardous waste and may be disposed as
construction waste to disposal or recycling.
The packaging properly emptied is not classified as hazardous waste.
LCA: Scenarios and additional technical information
The following information describe the scenarios in the different modules of the EPD.
Transport from production place to user (A4)
Capacity
Fuel/Energy
Type utilisation (incl. Type of vehicle Distance km Unit Value (l/t)
consumption
return) %
Truck, lorry over
Truck 55,0 % 32 tonnes, EURO 152 0,022823 l/tkm 3,47
5
Railway l/tkm
Boat l/tkm
Other Transportation l/tkm
LCA: Results
System boundaries (X=included, MND=module not declared, MNR=module not relevant)
Construction Beyond the
Product stage installation User stage End of life stage . system
stage bondaries
A1 A2 A3 A4 A5 B1 B2 B3 B4 B5 B6 B7 C1 C2 C3 C4 . D
X X X X MND MND MND MND MND MND MND MND MND MND MND MND . MND
Environmental impact
Parameter Unit A1 A2 A3 A4
GWP kg CO 2 -eq 2,05E-01 1,48E-02 2,02E-02 1,33E-02
ODP kg CFC11 -eq 6,37E-09 2,27E-09 4,16E-09 2,58E-09
POCP kg C 2H 4-eq 4,32E-05 2,43E-06 6,18E-06 2,14E-06
AP kg SO 2 -eq 4,66E-04 5,00E-05 1,11E-04 4,31E-05
EP kg PO3- -eq 1,33E-04 8,52E-06 2,45E-05 7,23E-06
4
ADPM kg Sb -eq 5,45E-07 4,36E-08 1,97E-08 2,99E-08
ADPE MJ 2,58E+00 2,24E-01 3,23E-01 2,08E-01
GWP Global warming potential; ODP Depletion potential of the stratospheric ozone layer; POCP Formation potential of tropospheric photochemical
oxidants; AP Acidification potential of land and water; EP Eutrophication potential; ADPM Abiotic depletion potential for non fossil resources; ADPE
Abiotic depletion potential for fossil resources
Reading example: 9,0 E-03 = 9,0*10-3 = 0,009
*INA Indicator Not Assessed
waR slairetam tropsnarT
gnirutcafunaM
tropsnarT ylbmessA esU ecnanetniaM riapeR tnemecalpeR
tnemhsibrufeR
lanoitarepO ygrene esu lanoitarepO esu retaw -eD noitcurtsnoc noitilomed tropsnarT etsaW gnissecorp lasopsiD
-yrevoceR-esueR
-gnilcyceR laitnetop
NEPD-2024-895-EN webertherm 261 putsbruk EF 3 / 8
Resource use
Parameter Unit A1 A2 A3 A4
RPEE MJ 3,52E-01 3,32E-03 2,63E-01 3,76E-03
RPEM MJ 1,02E-01 0,00E+00 0,00E+00 0,00E+00
TPE MJ 4,54E-01 3,32E-03 2,63E-01 3,76E-03
NRPE MJ 2,85E+00 2,30E-01 3,25E-01 2,14E-01
NRPM MJ 9,54E-02 0,00E+00 0,00E+00 0,00E+00
TRPE MJ 2,95E+00 2,30E-01 3,25E-01 2,14E-01
SM kg 8,71E-04 0,00E+00 0,00E+00 0,00E+00
RSF MJ 7,58E-02 0,00E+00 0,00E+00 0,00E+00
NRSF MJ 1,04E-01 0,00E+00 0,00E+00 0,00E+00
W m3 2,72E-03 4,66E-05 4,04E-05 5,05E-05
RPEE Renewable primary energy resources used as energy carrier; RPEM Renewable primary energy resources used as raw materials; TPE Total use
of renewable primary energy resources; NRPE Non renewable primary energy resources used as energy carrier; NRPM Non renewable primary energy
resources used as materials; TRPE Total use of non renewable primary energy resources; SM Use of secondary materials; RSF Use of renewable
secondary fuels; NRSF Use of non renewable secondary fuels; W Use of net fresh water
Reading example: 9,0 E-03 = 9,0*10-3 = 0,009
*INA Indicator Not Assessed
End of life - Waste
Parameter Unit A1 A2 A3 A4
HW kg 1,76E-06 1,37E-07 2,28E-05 1,14E-07
NHW kg 1,99E-02 1,31E-02 6,81E-02 1,95E-02
RW kg INA* INA* INA* INA*
HW Hazardous waste disposed; NHW Non hazardous waste disposed; RW Radioactive waste disposed
Reading example: 9,0 E-03 = 9,0*10-3 = 0,009
*INA Indicator Not Assessed
End of life - Output flow
Parameter Unit A1 A2 A3 A4
CR kg 0,00E+00 0,00E+00 0,00E+00 0,00E+00
MR kg 7,84E-08 0,00E+00 3,68E-04 0,00E+00
MER kg 3,21E-06 0,00E+00 1,55E-03 0,00E+00
EEE MJ INA* INA* INA* INA*
ETE MJ INA* INA* INA* INA*
CR Components for reuse; MR Materials for recycling; MER Materials for energy recovery; EEE Exported electric energy; ETE Exported thermal
energy
Reading example: 9,0 E-03 = 9,0*10-3 = 0,009
*INA Indicator Not Assessed
Additional Norwegian requirements
Greenhouse gas emissions from the use of electricity in the manufacturing phase
National production mix from import, low voltage (production of transmission lines, in addition to direct emissions and losses in grid) of applied
electricity for the manufacturing process (A3).
Electricity mix Data source Amount Unit
Renewable electricity with Guarantee of Origin from LOS (kWh) Modified ecoinvent 3.4 60,20 g CO2-ekv/kWh
Dangerous substances
The product contains no substances given by the REACH Candidate list or the Norwegian priority list. The product is classified as hazardous waste
(Avfallsforskriften, Annex III), see table.
Name CASNo Amount
Portand Cement 65997-15-1 10-20%
Indoor environment
The product has no impact on the indoor environment.
Bibliography
ISO 14025:2010 Environmental labels and declarations - Type III environmental declarations - Principles and procedures.
ISO 14044:2006 Environmental management - Life cycle assessment - Requirements and guidelines.
EN 15804:2012+A1:2013 Environmental product declaration - Core rules for the product category of construction products.
ISO 21930:2017 Sustainability in buildings and civil engineering works. Core rules for environmental product declarations of construction products.
ecoinvent v3, Allocation, cut-off by classification, Swiss Centre of Life Cycle Inventories.
Iversen et al., (2018) eEPD v3.0 - Background information for EPD generator system, LCA.no report number 04.18
Iversen et al., (2019) EPD generator for Saint-Gobain Weber and Scanspac - Background information and LCA data, LCA.no report number 05.18
NPCR Part A: Construction products and services. Ver. 1.0. April 2017, EPD-Norge.
NPCR 009 Part B for technical-chemical products. Ver. 1.0 June 2018, EPD-Norge.
Product Category Rules for Environmental Product Declarations: Institut Bauen und Umwelt e.V. (IBU): Requirements on the EPD for Mineral
factorymade
mortar.
Program operator and publisher Phone: +47 97722020
The Norwegian EPD Foundation
Post Box 5250 Majorstuen, 0303 Oslo e-mail: post@epd-norge.no
0303 Oslo Norway web: www.epd-norge.no
Owner of the declaration Phone: +46 8 625 6105
Saint-Gobain Sweden AB, Weber Fax:
Box 415 e-mail: anders.anderberg@weber.se
SE-19162 Sollentuna web: www.weber.se
Author of the Life Cycle Assessment Phone: +47 916 50 916
LCA.no AS Fax:
Dokka 1C e-mail: post@lca.no
1671 Kråkerøy web: www.lca.no
Developer of EPD generator Phone: +47 916 50 916
LCA.no AS
Dokka 1C e-mail: post@lca.no
1671 Kråkerøy web: www.lca.no
ver1 2015
ENVIRONMENTAL PRODUCT DECLARATION
in accordance with ISO 14025, ISO 21930 and EN 15804
Owner of the declaration: Saint-Gobain Sweden AB, Weber
Program operator: The Norwegian EPD Foundation
The Norwegian EPD Foundation
Publisher:
Declaration number: NEPD-2024-895-EN
Registration number: NEPD-2024-895-EN
ECO Platform reference number: -
Issue date: 23.01.2020
Valid to: 23.01.2025
webertherm 261 putsbruk EF
Saint-Gobain Sweden AB, Weber
www.epd-norge.no
General information
Product: Owner of the declaration:
webertherm 261 putsbruk EF Saint-Gobain Sweden AB, Weber
Contact person: Anders Anderberg
Phone: +46 8 625 6105
e-mail: anders.anderberg@weber.se
Program operator: Manufacturer:
The Norwegian EPD Foundation Saint-Gobain Sweden AB, Weber
Pb. 5250 Majorstuen, 0303 Oslo
Phone: +47 97722020
e-mail: post@epd-norge.no
Declaration number: Place of production:
NEPD-2024-895-EN Saint-Gobain Sweden AB, Weber, Riksten
ECO Platform reference number: Management system:
ISO 9001, ISO 14001
This declaration is based on Product Category Rules: Organisation no:
CEN Standard EN 15804:2012+A1:2013 serves as core PCR. SE-556241-2592
Requirements on the EPD for Mineral factory-made mortar.
Statement of liability: Issue date: 23.01.2020
The owner of the declaration shall be liable for the underlying
information and evidence. EPD Norway shall not be liable with Valid to: 23.01.2025
respect to manufacturer information, life cycle assessment data and
evidences.
Declared unit: Year of study:
1 kg webertherm 261 putsbruk EF 2018
Declared unit with option: Comparability:
EPD of construction products may not be comparable if they not
A1,A2,A3,A4
comply with EN 15804 and seen in a building context.
Functional unit: Author of the Life Cycle Assessment:
The declaration is developed using eEPD v3.0 from LCA.no
Approval:
Company specific data are:
Collected/registered by: Charlotte Karlsson
Internal verification by: Helene Wallgren
Verification: Approved:
Independent verification of data, other environmental information and
the declaration according to ISO14025:2010, § 8.1.3 and § 8.1.4
External
Third party verifier:
Sign Sign
Senior Research Scientist, Anne Rønning
(Independent verifier approved by EPD Norway)
Product
Product description: Technical data:
webertherm 261 putsbruk EF is a factory-made fiber-reinforced dry mortar webertherm 261 putsbruk EF is tested and approved according to EN 998-
based on lime and cement with natural sand as aggregates. When mixed 1 and ETA SP 105 Fire.
with water, it is a ready-to-use render for indor and outdoor use.
webertherm 261 putsbruk EF is a hydrofobic render specially designed for Mortar category: CS III.
use in Serpomin EF facade systems and Serpovent G2. webertherm 261
putsbruk EF can also be used on both Exclay,bricks and Concrete as well For further information, see www.se.weber/
as previously renderd facades. webertherm 261 putsbruk EF is applied in
Market:
two layers, the first layer (> 6mm), and the second layer around 2-3 mm.
The render is sprayable and pumpable in a 60m hose. Sweden and Denmark
Reference service life, product
webertherm 261 putsbruk EF can be delivered in closed silos of 10 tons
with a flow mixer to avoid dust. The reference service life of the product is similar to the service life of the
building.
Product specification
Reference service life, building
50 years.
Materials %
Binder 10-30
Aggregate 60-90
Filler 5-10
Additives <5
Packaging <0,2
LCA: Calculation rules
Declared unit: Allocation:
The allocation is made in accordance with the provisions of EN 15804.
1 kg webertherm 261 putsbruk EF
Incoming energy and water and waste production in-house is allocated
Cut-off criteria: equally among all products through mass allocation. Effects of primary
All major raw materials and all the essential energy is included. The production of recycled materials is allocated to the main product in which
production processes for raw materials and energy flows with very small the material was used. The recycling process and transportation of the
amounts (less than 1%) are not included. These cut-off criteria do not material is allocated to this analysis.
apply for hazardous materials and substances.
Data quality:
Specific data for the product composition are provided by the manufacturer. They represent the production of the declared product and were collected
for EPD development in the year of study. Background data is based on registered EPDs according to EN 15804, Ostfold Research databases,
ecoinvent and other LCA databases. The data quality of the raw materials in A1 is presented in the table below.
Materials Source Data quality Year
Cement Supplier EPD 2014
Additives ecoinvent 3.4 Database 2017
Aggregate ecoinvent 3.4 Database 2017
Filler ecoinvent 3.4 Database 2017
Packaging ecoinvent 3.4 Database 2017
Packaging Modified ecoinvent 3.4 Database 2017
SC 99 Owner of EPD Database
SC 354 Owner of EPD Database 2018
SC 425 Owner of EPD Database 2019
System boundary:
"All processes from raw material extraction to product from the factory gate are included in the analysis (A1-A3). In addition, transportation to a central
warehouse placed in accordance with guidelines issued by the EPD Norway (A4) is included.
The flow chart below illustrates the system boundaries for the A1 to A3 part of the analysis."
Additional technical information:
webertherm 261 putsbruk EF is a render in the ventilated Serpovent G2 , Serpovent G2 has been verified for fire according to SP 105 Fire.
The remaining powder is classified as hazardous waste. Cured material is inactive and not classified as hazardous waste and may be disposed as
construction waste to disposal or recycling.
The packaging properly emptied is not classified as hazardous waste.
LCA: Scenarios and additional technical information
The following information describe the scenarios in the different modules of the EPD.
Transport from production place to user (A4)
Capacity
Fuel/Energy
Type utilisation (incl. Type of vehicle Distance km Unit Value (l/t)
consumption
return) %
Truck, lorry over
Truck 55,0 % 32 tonnes, EURO 152 0,022823 l/tkm 3,47
5
Railway l/tkm
Boat l/tkm
Other Transportation l/tkm
LCA: Results
System boundaries (X=included, MND=module not declared, MNR=module not relevant)
Construction Beyond the
Product stage installation User stage End of life stage . system
stage bondaries
A1 A2 A3 A4 A5 B1 B2 B3 B4 B5 B6 B7 C1 C2 C3 C4 . D
X X X X MND MND MND MND MND MND MND MND MND MND MND MND . MND
Environmental impact
Parameter Unit A1 A2 A3 A4
GWP kg CO 2 -eq 2,05E-01 1,48E-02 2,02E-02 1,33E-02
ODP kg CFC11 -eq 6,37E-09 2,27E-09 4,16E-09 2,58E-09
POCP kg C 2H 4-eq 4,32E-05 2,43E-06 6,18E-06 2,14E-06
AP kg SO 2 -eq 4,66E-04 5,00E-05 1,11E-04 4,31E-05
EP kg PO3- -eq 1,33E-04 8,52E-06 2,45E-05 7,23E-06
4
ADPM kg Sb -eq 5,45E-07 4,36E-08 1,97E-08 2,99E-08
ADPE MJ 2,58E+00 2,24E-01 3,23E-01 2,08E-01
GWP Global warming potential; ODP Depletion potential of the stratospheric ozone layer; POCP Formation potential of tropospheric photochemical
oxidants; AP Acidification potential of land and water; EP Eutrophication potential; ADPM Abiotic depletion potential for non fossil resources; ADPE
Abiotic depletion potential for fossil resources
Reading example: 9,0 E-03 = 9,0*10-3 = 0,009
*INA Indicator Not Assessed
waR slairetam tropsnarT
gnirutcafunaM
tropsnarT ylbmessA esU ecnanetniaM riapeR tnemecalpeR
tnemhsibrufeR
lanoitarepO ygrene esu lanoitarepO esu retaw -eD noitcurtsnoc noitilomed tropsnarT etsaW gnissecorp lasopsiD
-yrevoceR-esueR
-gnilcyceR laitnetop
NEPD-2024-895-EN webertherm 261 putsbruk EF 4 / 8
Resource use
Parameter Unit A1 A2 A3 A4
RPEE MJ 3,52E-01 3,32E-03 2,63E-01 3,76E-03
RPEM MJ 1,02E-01 0,00E+00 0,00E+00 0,00E+00
TPE MJ 4,54E-01 3,32E-03 2,63E-01 3,76E-03
NRPE MJ 2,85E+00 2,30E-01 3,25E-01 2,14E-01
NRPM MJ 9,54E-02 0,00E+00 0,00E+00 0,00E+00
TRPE MJ 2,95E+00 2,30E-01 3,25E-01 2,14E-01
SM kg 8,71E-04 0,00E+00 0,00E+00 0,00E+00
RSF MJ 7,58E-02 0,00E+00 0,00E+00 0,00E+00
NRSF MJ 1,04E-01 0,00E+00 0,00E+00 0,00E+00
W m3 2,72E-03 4,66E-05 4,04E-05 5,05E-05
RPEE Renewable primary energy resources used as energy carrier; RPEM Renewable primary energy resources used as raw materials; TPE Total use
of renewable primary energy resources; NRPE Non renewable primary energy resources used as energy carrier; NRPM Non renewable primary energy
resources used as materials; TRPE Total use of non renewable primary energy resources; SM Use of secondary materials; RSF Use of renewable
secondary fuels; NRSF Use of non renewable secondary fuels; W Use of net fresh water
Reading example: 9,0 E-03 = 9,0*10-3 = 0,009
*INA Indicator Not Assessed
End of life - Waste
Parameter Unit A1 A2 A3 A4
HW kg 1,76E-06 1,37E-07 2,28E-05 1,14E-07
NHW kg 1,99E-02 1,31E-02 6,81E-02 1,95E-02
RW kg INA* INA* INA* INA*
HW Hazardous waste disposed; NHW Non hazardous waste disposed; RW Radioactive waste disposed
Reading example: 9,0 E-03 = 9,0*10-3 = 0,009
*INA Indicator Not Assessed
End of life - Output flow
Parameter Unit A1 A2 A3 A4
CR kg 0,00E+00 0,00E+00 0,00E+00 0,00E+00
MR kg 7,84E-08 0,00E+00 3,68E-04 0,00E+00
MER kg 3,21E-06 0,00E+00 1,55E-03 0,00E+00
EEE MJ INA* INA* INA* INA*
ETE MJ INA* INA* INA* INA*
CR Components for reuse; MR Materials for recycling; MER Materials for energy recovery; EEE Exported electric energy; ETE Exported thermal
energy
Reading example: 9,0 E-03 = 9,0*10-3 = 0,009
*INA Indicator Not Assessed
Additional Norwegian requirements
Greenhouse gas emissions from the use of electricity in the manufacturing phase
National production mix from import, low voltage (production of transmission lines, in addition to direct emissions and losses in grid) of applied
electricity for the manufacturing process (A3).
Electricity mix Data source Amount Unit
Renewable electricity with Guarantee of Origin from LOS (kWh) Modified ecoinvent 3.4 60,20 g CO2-ekv/kWh
Dangerous substances
The product contains no substances given by the REACH Candidate list or the Norwegian priority list. The product is classified as hazardous waste
(Avfallsforskriften, Annex III), see table.
Name CASNo Amount
Portand Cement 65997-15-1 10-20%
Indoor environment
The product has no impact on the indoor environment.
Bibliography
ISO 14025:2010 Environmental labels and declarations - Type III environmental declarations - Principles and procedures.
ISO 14044:2006 Environmental management - Life cycle assessment - Requirements and guidelines.
EN 15804:2012+A1:2013 Environmental product declaration - Core rules for the product category of construction products.
ISO 21930:2017 Sustainability in buildings and civil engineering works. Core rules for environmental product declarations of construction products.
ecoinvent v3, Allocation, cut-off by classification, Swiss Centre of Life Cycle Inventories.
Iversen et al., (2018) eEPD v3.0 - Background information for EPD generator system, LCA.no report number 04.18
Iversen et al., (2019) EPD generator for Saint-Gobain Weber and Scanspac - Background information and LCA data, LCA.no report number 05.18
NPCR Part A: Construction products and services. Ver. 1.0. April 2017, EPD-Norge.
NPCR 009 Part B for technical-chemical products. Ver. 1.0 June 2018, EPD-Norge.
Product Category Rules for Environmental Product Declarations: Institut Bauen und Umwelt e.V. (IBU): Requirements on the EPD for Mineral
factorymade
mortar.
Program operator and publisher Phone: +47 97722020
The Norwegian EPD Foundation
Post Box 5250 Majorstuen, 0303 Oslo e-mail: post@epd-norge.no
0303 Oslo Norway web: www.epd-norge.no
Owner of the declaration Phone: +46 8 625 6105
Saint-Gobain Sweden AB, Weber Fax:
Box 415 e-mail: anders.anderberg@weber.se
SE-19162 Sollentuna web: www.weber.se
Author of the Life Cycle Assessment Phone: +47 916 50 916
LCA.no AS Fax:
Dokka 1C e-mail: post@lca.no
1671 Kråkerøy web: www.lca.no
Developer of EPD generator Phone: +47 916 50 916
LCA.no AS
Dokka 1C e-mail: post@lca.no
1671 Kråkerøy web: www.lca.no
ver1 2015
ENVIRONMENTAL PRODUCT DECLARATION
in accordance with ISO 14025, ISO 21930 and EN 15804
Owner of the declaration: Saint-Gobain Sweden AB, Weber
Program operator: The Norwegian EPD Foundation
The Norwegian EPD Foundation
Publisher:
Declaration number: NEPD-2024-895-EN
Registration number: NEPD-2024-895-EN
ECO Platform reference number: -
Issue date: 23.01.2020
Valid to: 23.01.2025
webertherm 261 putsbruk EF
Saint-Gobain Sweden AB, Weber
www.epd-norge.no
General information
Product: Owner of the declaration:
webertherm 261 putsbruk EF Saint-Gobain Sweden AB, Weber
Contact person: Anders Anderberg
Phone: +46 8 625 6105
e-mail: anders.anderberg@weber.se
Program operator: Manufacturer:
The Norwegian EPD Foundation Saint-Gobain Sweden AB, Weber
Pb. 5250 Majorstuen, 0303 Oslo
Phone: +47 97722020
e-mail: post@epd-norge.no
Declaration number: Place of production:
NEPD-2024-895-EN Saint-Gobain Sweden AB, Weber, Riksten
ECO Platform reference number: Management system:
ISO 9001, ISO 14001
This declaration is based on Product Category Rules: Organisation no:
CEN Standard EN 15804:2012+A1:2013 serves as core PCR. SE-556241-2592
Requirements on the EPD for Mineral factory-made mortar.
Statement of liability: Issue date: 23.01.2020
The owner of the declaration shall be liable for the underlying
information and evidence. EPD Norway shall not be liable with Valid to: 23.01.2025
respect to manufacturer information, life cycle assessment data and
evidences.
Declared unit: Year of study:
1 kg webertherm 261 putsbruk EF 2018
Declared unit with option: Comparability:
EPD of construction products may not be comparable if they not
A1,A2,A3,A4
comply with EN 15804 and seen in a building context.
Functional unit: Author of the Life Cycle Assessment:
The declaration is developed using eEPD v3.0 from LCA.no
Approval:
Company specific data are:
Collected/registered by: Charlotte Karlsson
Internal verification by: Helene Wallgren
Verification: Approved:
Independent verification of data, other environmental information and
the declaration according to ISO14025:2010, § 8.1.3 and § 8.1.4
External
Third party verifier:
Sign Sign
Senior Research Scientist, Anne Rønning
(Independent verifier approved by EPD Norway)
Product
Product description: Technical data:
webertherm 261 putsbruk EF is a factory-made fiber-reinforced dry mortar webertherm 261 putsbruk EF is tested and approved according to EN 998-
based on lime and cement with natural sand as aggregates. When mixed 1 and ETA SP 105 Fire.
with water, it is a ready-to-use render for indor and outdoor use.
webertherm 261 putsbruk EF is a hydrofobic render specially designed for Mortar category: CS III.
use in Serpomin EF facade systems and Serpovent G2. webertherm 261
putsbruk EF can also be used on both Exclay,bricks and Concrete as well For further information, see www.se.weber/
as previously renderd facades. webertherm 261 putsbruk EF is applied in
Market:
two layers, the first layer (> 6mm), and the second layer around 2-3 mm.
The render is sprayable and pumpable in a 60m hose. Sweden and Denmark
Reference service life, product
webertherm 261 putsbruk EF can be delivered in closed silos of 10 tons
with a flow mixer to avoid dust. The reference service life of the product is similar to the service life of the
building.
Product specification
Reference service life, building
50 years.
Materials %
Binder 10-30
Aggregate 60-90
Filler 5-10
Additives <5
Packaging <0,2
LCA: Calculation rules
Declared unit: Allocation:
The allocation is made in accordance with the provisions of EN 15804.
1 kg webertherm 261 putsbruk EF
Incoming energy and water and waste production in-house is allocated
Cut-off criteria: equally among all products through mass allocation. Effects of primary
All major raw materials and all the essential energy is included. The production of recycled materials is allocated to the main product in which
production processes for raw materials and energy flows with very small the material was used. The recycling process and transportation of the
amounts (less than 1%) are not included. These cut-off criteria do not material is allocated to this analysis.
apply for hazardous materials and substances.
Data quality:
Specific data for the product composition are provided by the manufacturer. They represent the production of the declared product and were collected
for EPD development in the year of study. Background data is based on registered EPDs according to EN 15804, Ostfold Research databases,
ecoinvent and other LCA databases. The data quality of the raw materials in A1 is presented in the table below.
Materials Source Data quality Year
Cement Supplier EPD 2014
Additives ecoinvent 3.4 Database 2017
Aggregate ecoinvent 3.4 Database 2017
Filler ecoinvent 3.4 Database 2017
Packaging ecoinvent 3.4 Database 2017
Packaging Modified ecoinvent 3.4 Database 2017
SC 99 Owner of EPD Database
SC 354 Owner of EPD Database 2018
SC 425 Owner of EPD Database 2019
System boundary:
"All processes from raw material extraction to product from the factory gate are included in the analysis (A1-A3). In addition, transportation to a central
warehouse placed in accordance with guidelines issued by the EPD Norway (A4) is included.
The flow chart below illustrates the system boundaries for the A1 to A3 part of the analysis."
Additional technical information:
webertherm 261 putsbruk EF is a render in the ventilated Serpovent G2 , Serpovent G2 has been verified for fire according to SP 105 Fire.
The remaining powder is classified as hazardous waste. Cured material is inactive and not classified as hazardous waste and may be disposed as
construction waste to disposal or recycling.
The packaging properly emptied is not classified as hazardous waste.
LCA: Scenarios and additional technical information
The following information describe the scenarios in the different modules of the EPD.
Transport from production place to user (A4)
Capacity
Fuel/Energy
Type utilisation (incl. Type of vehicle Distance km Unit Value (l/t)
consumption
return) %
Truck, lorry over
Truck 55,0 % 32 tonnes, EURO 152 0,022823 l/tkm 3,47
5
Railway l/tkm
Boat l/tkm
Other Transportation l/tkm
LCA: Results
System boundaries (X=included, MND=module not declared, MNR=module not relevant)
Construction Beyond the
Product stage installation User stage End of life stage . system
stage bondaries
A1 A2 A3 A4 A5 B1 B2 B3 B4 B5 B6 B7 C1 C2 C3 C4 . D
X X X X MND MND MND MND MND MND MND MND MND MND MND MND . MND
Environmental impact
Parameter Unit A1 A2 A3 A4
GWP kg CO 2 -eq 2,05E-01 1,48E-02 2,02E-02 1,33E-02
ODP kg CFC11 -eq 6,37E-09 2,27E-09 4,16E-09 2,58E-09
POCP kg C 2H 4-eq 4,32E-05 2,43E-06 6,18E-06 2,14E-06
AP kg SO 2 -eq 4,66E-04 5,00E-05 1,11E-04 4,31E-05
EP kg PO3- -eq 1,33E-04 8,52E-06 2,45E-05 7,23E-06
4
ADPM kg Sb -eq 5,45E-07 4,36E-08 1,97E-08 2,99E-08
ADPE MJ 2,58E+00 2,24E-01 3,23E-01 2,08E-01
GWP Global warming potential; ODP Depletion potential of the stratospheric ozone layer; POCP Formation potential of tropospheric photochemical
oxidants; AP Acidification potential of land and water; EP Eutrophication potential; ADPM Abiotic depletion potential for non fossil resources; ADPE
Abiotic depletion potential for fossil resources
Reading example: 9,0 E-03 = 9,0*10-3 = 0,009
*INA Indicator Not Assessed
waR slairetam tropsnarT
gnirutcafunaM
tropsnarT ylbmessA esU ecnanetniaM riapeR tnemecalpeR
tnemhsibrufeR
lanoitarepO ygrene esu lanoitarepO esu retaw -eD noitcurtsnoc noitilomed tropsnarT etsaW gnissecorp lasopsiD
-yrevoceR-esueR
-gnilcyceR laitnetop
NEPD-2024-895-EN webertherm 261 putsbruk EF 5 / 8
Resource use
Parameter Unit A1 A2 A3 A4
RPEE MJ 3,52E-01 3,32E-03 2,63E-01 3,76E-03
RPEM MJ 1,02E-01 0,00E+00 0,00E+00 0,00E+00
TPE MJ 4,54E-01 3,32E-03 2,63E-01 3,76E-03
NRPE MJ 2,85E+00 2,30E-01 3,25E-01 2,14E-01
NRPM MJ 9,54E-02 0,00E+00 0,00E+00 0,00E+00
TRPE MJ 2,95E+00 2,30E-01 3,25E-01 2,14E-01
SM kg 8,71E-04 0,00E+00 0,00E+00 0,00E+00
RSF MJ 7,58E-02 0,00E+00 0,00E+00 0,00E+00
NRSF MJ 1,04E-01 0,00E+00 0,00E+00 0,00E+00
W m3 2,72E-03 4,66E-05 4,04E-05 5,05E-05
RPEE Renewable primary energy resources used as energy carrier; RPEM Renewable primary energy resources used as raw materials; TPE Total use
of renewable primary energy resources; NRPE Non renewable primary energy resources used as energy carrier; NRPM Non renewable primary energy
resources used as materials; TRPE Total use of non renewable primary energy resources; SM Use of secondary materials; RSF Use of renewable
secondary fuels; NRSF Use of non renewable secondary fuels; W Use of net fresh water
Reading example: 9,0 E-03 = 9,0*10-3 = 0,009
*INA Indicator Not Assessed
End of life - Waste
Parameter Unit A1 A2 A3 A4
HW kg 1,76E-06 1,37E-07 2,28E-05 1,14E-07
NHW kg 1,99E-02 1,31E-02 6,81E-02 1,95E-02
RW kg INA* INA* INA* INA*
HW Hazardous waste disposed; NHW Non hazardous waste disposed; RW Radioactive waste disposed
Reading example: 9,0 E-03 = 9,0*10-3 = 0,009
*INA Indicator Not Assessed
End of life - Output flow
Parameter Unit A1 A2 A3 A4
CR kg 0,00E+00 0,00E+00 0,00E+00 0,00E+00
MR kg 7,84E-08 0,00E+00 3,68E-04 0,00E+00
MER kg 3,21E-06 0,00E+00 1,55E-03 0,00E+00
EEE MJ INA* INA* INA* INA*
ETE MJ INA* INA* INA* INA*
CR Components for reuse; MR Materials for recycling; MER Materials for energy recovery; EEE Exported electric energy; ETE Exported thermal
energy
Reading example: 9,0 E-03 = 9,0*10-3 = 0,009
*INA Indicator Not Assessed
Additional Norwegian requirements
Greenhouse gas emissions from the use of electricity in the manufacturing phase
National production mix from import, low voltage (production of transmission lines, in addition to direct emissions and losses in grid) of applied
electricity for the manufacturing process (A3).
Electricity mix Data source Amount Unit
Renewable electricity with Guarantee of Origin from LOS (kWh) Modified ecoinvent 3.4 60,20 g CO2-ekv/kWh
Dangerous substances
The product contains no substances given by the REACH Candidate list or the Norwegian priority list. The product is classified as hazardous waste
(Avfallsforskriften, Annex III), see table.
Name CASNo Amount
Portand Cement 65997-15-1 10-20%
Indoor environment
The product has no impact on the indoor environment.
Bibliography
ISO 14025:2010 Environmental labels and declarations - Type III environmental declarations - Principles and procedures.
ISO 14044:2006 Environmental management - Life cycle assessment - Requirements and guidelines.
EN 15804:2012+A1:2013 Environmental product declaration - Core rules for the product category of construction products.
ISO 21930:2017 Sustainability in buildings and civil engineering works. Core rules for environmental product declarations of construction products.
ecoinvent v3, Allocation, cut-off by classification, Swiss Centre of Life Cycle Inventories.
Iversen et al., (2018) eEPD v3.0 - Background information for EPD generator system, LCA.no report number 04.18
Iversen et al., (2019) EPD generator for Saint-Gobain Weber and Scanspac - Background information and LCA data, LCA.no report number 05.18
NPCR Part A: Construction products and services. Ver. 1.0. April 2017, EPD-Norge.
NPCR 009 Part B for technical-chemical products. Ver. 1.0 June 2018, EPD-Norge.
Product Category Rules for Environmental Product Declarations: Institut Bauen und Umwelt e.V. (IBU): Requirements on the EPD for Mineral
factorymade
mortar.
Program operator and publisher Phone: +47 97722020
The Norwegian EPD Foundation
Post Box 5250 Majorstuen, 0303 Oslo e-mail: post@epd-norge.no
0303 Oslo Norway web: www.epd-norge.no
Owner of the declaration Phone: +46 8 625 6105
Saint-Gobain Sweden AB, Weber Fax:
Box 415 e-mail: anders.anderberg@weber.se
SE-19162 Sollentuna web: www.weber.se
Author of the Life Cycle Assessment Phone: +47 916 50 916
LCA.no AS Fax:
Dokka 1C e-mail: post@lca.no
1671 Kråkerøy web: www.lca.no
Developer of EPD generator Phone: +47 916 50 916
LCA.no AS
Dokka 1C e-mail: post@lca.no
1671 Kråkerøy web: www.lca.no
ver1 2015
ENVIRONMENTAL PRODUCT DECLARATION
in accordance with ISO 14025, ISO 21930 and EN 15804
Owner of the declaration: Saint-Gobain Sweden AB, Weber
Program operator: The Norwegian EPD Foundation
The Norwegian EPD Foundation
Publisher:
Declaration number: NEPD-2024-895-EN
Registration number: NEPD-2024-895-EN
ECO Platform reference number: -
Issue date: 23.01.2020
Valid to: 23.01.2025
webertherm 261 putsbruk EF
Saint-Gobain Sweden AB, Weber
www.epd-norge.no
General information
Product: Owner of the declaration:
webertherm 261 putsbruk EF Saint-Gobain Sweden AB, Weber
Contact person: Anders Anderberg
Phone: +46 8 625 6105
e-mail: anders.anderberg@weber.se
Program operator: Manufacturer:
The Norwegian EPD Foundation Saint-Gobain Sweden AB, Weber
Pb. 5250 Majorstuen, 0303 Oslo
Phone: +47 97722020
e-mail: post@epd-norge.no
Declaration number: Place of production:
NEPD-2024-895-EN Saint-Gobain Sweden AB, Weber, Riksten
ECO Platform reference number: Management system:
ISO 9001, ISO 14001
This declaration is based on Product Category Rules: Organisation no:
CEN Standard EN 15804:2012+A1:2013 serves as core PCR. SE-556241-2592
Requirements on the EPD for Mineral factory-made mortar.
Statement of liability: Issue date: 23.01.2020
The owner of the declaration shall be liable for the underlying
information and evidence. EPD Norway shall not be liable with Valid to: 23.01.2025
respect to manufacturer information, life cycle assessment data and
evidences.
Declared unit: Year of study:
1 kg webertherm 261 putsbruk EF 2018
Declared unit with option: Comparability:
EPD of construction products may not be comparable if they not
A1,A2,A3,A4
comply with EN 15804 and seen in a building context.
Functional unit: Author of the Life Cycle Assessment:
The declaration is developed using eEPD v3.0 from LCA.no
Approval:
Company specific data are:
Collected/registered by: Charlotte Karlsson
Internal verification by: Helene Wallgren
Verification: Approved:
Independent verification of data, other environmental information and
the declaration according to ISO14025:2010, § 8.1.3 and § 8.1.4
External
Third party verifier:
Sign Sign
Senior Research Scientist, Anne Rønning
(Independent verifier approved by EPD Norway)
Product
Product description: Technical data:
webertherm 261 putsbruk EF is a factory-made fiber-reinforced dry mortar webertherm 261 putsbruk EF is tested and approved according to EN 998-
based on lime and cement with natural sand as aggregates. When mixed 1 and ETA SP 105 Fire.
with water, it is a ready-to-use render for indor and outdoor use.
webertherm 261 putsbruk EF is a hydrofobic render specially designed for Mortar category: CS III.
use in Serpomin EF facade systems and Serpovent G2. webertherm 261
putsbruk EF can also be used on both Exclay,bricks and Concrete as well For further information, see www.se.weber/
as previously renderd facades. webertherm 261 putsbruk EF is applied in
Market:
two layers, the first layer (> 6mm), and the second layer around 2-3 mm.
The render is sprayable and pumpable in a 60m hose. Sweden and Denmark
Reference service life, product
webertherm 261 putsbruk EF can be delivered in closed silos of 10 tons
with a flow mixer to avoid dust. The reference service life of the product is similar to the service life of the
building.
Product specification
Reference service life, building
50 years.
Materials %
Binder 10-30
Aggregate 60-90
Filler 5-10
Additives <5
Packaging <0,2
LCA: Calculation rules
Declared unit: Allocation:
The allocation is made in accordance with the provisions of EN 15804.
1 kg webertherm 261 putsbruk EF
Incoming energy and water and waste production in-house is allocated
Cut-off criteria: equally among all products through mass allocation. Effects of primary
All major raw materials and all the essential energy is included. The production of recycled materials is allocated to the main product in which
production processes for raw materials and energy flows with very small the material was used. The recycling process and transportation of the
amounts (less than 1%) are not included. These cut-off criteria do not material is allocated to this analysis.
apply for hazardous materials and substances.
Data quality:
Specific data for the product composition are provided by the manufacturer. They represent the production of the declared product and were collected
for EPD development in the year of study. Background data is based on registered EPDs according to EN 15804, Ostfold Research databases,
ecoinvent and other LCA databases. The data quality of the raw materials in A1 is presented in the table below.
Materials Source Data quality Year
Cement Supplier EPD 2014
Additives ecoinvent 3.4 Database 2017
Aggregate ecoinvent 3.4 Database 2017
Filler ecoinvent 3.4 Database 2017
Packaging ecoinvent 3.4 Database 2017
Packaging Modified ecoinvent 3.4 Database 2017
SC 99 Owner of EPD Database
SC 354 Owner of EPD Database 2018
SC 425 Owner of EPD Database 2019
System boundary:
"All processes from raw material extraction to product from the factory gate are included in the analysis (A1-A3). In addition, transportation to a central
warehouse placed in accordance with guidelines issued by the EPD Norway (A4) is included.
The flow chart below illustrates the system boundaries for the A1 to A3 part of the analysis."
Additional technical information:
webertherm 261 putsbruk EF is a render in the ventilated Serpovent G2 , Serpovent G2 has been verified for fire according to SP 105 Fire.
The remaining powder is classified as hazardous waste. Cured material is inactive and not classified as hazardous waste and may be disposed as
construction waste to disposal or recycling.
The packaging properly emptied is not classified as hazardous waste.
LCA: Scenarios and additional technical information
The following information describe the scenarios in the different modules of the EPD.
Transport from production place to user (A4)
Capacity
Fuel/Energy
Type utilisation (incl. Type of vehicle Distance km Unit Value (l/t)
consumption
return) %
Truck, lorry over
Truck 55,0 % 32 tonnes, EURO 152 0,022823 l/tkm 3,47
5
Railway l/tkm
Boat l/tkm
Other Transportation l/tkm
LCA: Results
System boundaries (X=included, MND=module not declared, MNR=module not relevant)
Construction Beyond the
Product stage installation User stage End of life stage . system
stage bondaries
A1 A2 A3 A4 A5 B1 B2 B3 B4 B5 B6 B7 C1 C2 C3 C4 . D
X X X X MND MND MND MND MND MND MND MND MND MND MND MND . MND
Environmental impact
Parameter Unit A1 A2 A3 A4
GWP kg CO 2 -eq 2,05E-01 1,48E-02 2,02E-02 1,33E-02
ODP kg CFC11 -eq 6,37E-09 2,27E-09 4,16E-09 2,58E-09
POCP kg C 2H 4-eq 4,32E-05 2,43E-06 6,18E-06 2,14E-06
AP kg SO 2 -eq 4,66E-04 5,00E-05 1,11E-04 4,31E-05
EP kg PO3- -eq 1,33E-04 8,52E-06 2,45E-05 7,23E-06
4
ADPM kg Sb -eq 5,45E-07 4,36E-08 1,97E-08 2,99E-08
ADPE MJ 2,58E+00 2,24E-01 3,23E-01 2,08E-01
GWP Global warming potential; ODP Depletion potential of the stratospheric ozone layer; POCP Formation potential of tropospheric photochemical
oxidants; AP Acidification potential of land and water; EP Eutrophication potential; ADPM Abiotic depletion potential for non fossil resources; ADPE
Abiotic depletion potential for fossil resources
Reading example: 9,0 E-03 = 9,0*10-3 = 0,009
*INA Indicator Not Assessed
waR slairetam tropsnarT
gnirutcafunaM
tropsnarT ylbmessA esU ecnanetniaM riapeR tnemecalpeR
tnemhsibrufeR
lanoitarepO ygrene esu lanoitarepO esu retaw -eD noitcurtsnoc noitilomed tropsnarT etsaW gnissecorp lasopsiD
-yrevoceR-esueR
-gnilcyceR laitnetop
NEPD-2024-895-EN webertherm 261 putsbruk EF 6 / 8
Resource use
Parameter Unit A1 A2 A3 A4
RPEE MJ 3,52E-01 3,32E-03 2,63E-01 3,76E-03
RPEM MJ 1,02E-01 0,00E+00 0,00E+00 0,00E+00
TPE MJ 4,54E-01 3,32E-03 2,63E-01 3,76E-03
NRPE MJ 2,85E+00 2,30E-01 3,25E-01 2,14E-01
NRPM MJ 9,54E-02 0,00E+00 0,00E+00 0,00E+00
TRPE MJ 2,95E+00 2,30E-01 3,25E-01 2,14E-01
SM kg 8,71E-04 0,00E+00 0,00E+00 0,00E+00
RSF MJ 7,58E-02 0,00E+00 0,00E+00 0,00E+00
NRSF MJ 1,04E-01 0,00E+00 0,00E+00 0,00E+00
W m3 2,72E-03 4,66E-05 4,04E-05 5,05E-05
RPEE Renewable primary energy resources used as energy carrier; RPEM Renewable primary energy resources used as raw materials; TPE Total use
of renewable primary energy resources; NRPE Non renewable primary energy resources used as energy carrier; NRPM Non renewable primary energy
resources used as materials; TRPE Total use of non renewable primary energy resources; SM Use of secondary materials; RSF Use of renewable
secondary fuels; NRSF Use of non renewable secondary fuels; W Use of net fresh water
Reading example: 9,0 E-03 = 9,0*10-3 = 0,009
*INA Indicator Not Assessed
End of life - Waste
Parameter Unit A1 A2 A3 A4
HW kg 1,76E-06 1,37E-07 2,28E-05 1,14E-07
NHW kg 1,99E-02 1,31E-02 6,81E-02 1,95E-02
RW kg INA* INA* INA* INA*
HW Hazardous waste disposed; NHW Non hazardous waste disposed; RW Radioactive waste disposed
Reading example: 9,0 E-03 = 9,0*10-3 = 0,009
*INA Indicator Not Assessed
End of life - Output flow
Parameter Unit A1 A2 A3 A4
CR kg 0,00E+00 0,00E+00 0,00E+00 0,00E+00
MR kg 7,84E-08 0,00E+00 3,68E-04 0,00E+00
MER kg 3,21E-06 0,00E+00 1,55E-03 0,00E+00
EEE MJ INA* INA* INA* INA*
ETE MJ INA* INA* INA* INA*
CR Components for reuse; MR Materials for recycling; MER Materials for energy recovery; EEE Exported electric energy; ETE Exported thermal
energy
Reading example: 9,0 E-03 = 9,0*10-3 = 0,009
*INA Indicator Not Assessed
Additional Norwegian requirements
Greenhouse gas emissions from the use of electricity in the manufacturing phase
National production mix from import, low voltage (production of transmission lines, in addition to direct emissions and losses in grid) of applied
electricity for the manufacturing process (A3).
Electricity mix Data source Amount Unit
Renewable electricity with Guarantee of Origin from LOS (kWh) Modified ecoinvent 3.4 60,20 g CO2-ekv/kWh
Dangerous substances
The product contains no substances given by the REACH Candidate list or the Norwegian priority list. The product is classified as hazardous waste
(Avfallsforskriften, Annex III), see table.
Name CASNo Amount
Portand Cement 65997-15-1 10-20%
Indoor environment
The product has no impact on the indoor environment.
Bibliography
ISO 14025:2010 Environmental labels and declarations - Type III environmental declarations - Principles and procedures.
ISO 14044:2006 Environmental management - Life cycle assessment - Requirements and guidelines.
EN 15804:2012+A1:2013 Environmental product declaration - Core rules for the product category of construction products.
ISO 21930:2017 Sustainability in buildings and civil engineering works. Core rules for environmental product declarations of construction products.
ecoinvent v3, Allocation, cut-off by classification, Swiss Centre of Life Cycle Inventories.
Iversen et al., (2018) eEPD v3.0 - Background information for EPD generator system, LCA.no report number 04.18
Iversen et al., (2019) EPD generator for Saint-Gobain Weber and Scanspac - Background information and LCA data, LCA.no report number 05.18
NPCR Part A: Construction products and services. Ver. 1.0. April 2017, EPD-Norge.
NPCR 009 Part B for technical-chemical products. Ver. 1.0 June 2018, EPD-Norge.
Product Category Rules for Environmental Product Declarations: Institut Bauen und Umwelt e.V. (IBU): Requirements on the EPD for Mineral
factorymade
mortar.
Program operator and publisher Phone: +47 97722020
The Norwegian EPD Foundation
Post Box 5250 Majorstuen, 0303 Oslo e-mail: post@epd-norge.no
0303 Oslo Norway web: www.epd-norge.no
Owner of the declaration Phone: +46 8 625 6105
Saint-Gobain Sweden AB, Weber Fax:
Box 415 e-mail: anders.anderberg@weber.se
SE-19162 Sollentuna web: www.weber.se
Author of the Life Cycle Assessment Phone: +47 916 50 916
LCA.no AS Fax:
Dokka 1C e-mail: post@lca.no
1671 Kråkerøy web: www.lca.no
Developer of EPD generator Phone: +47 916 50 916
LCA.no AS
Dokka 1C e-mail: post@lca.no
1671 Kråkerøy web: www.lca.no
ver1 2015
ENVIRONMENTAL PRODUCT DECLARATION
in accordance with ISO 14025, ISO 21930 and EN 15804
Owner of the declaration: Saint-Gobain Sweden AB, Weber
Program operator: The Norwegian EPD Foundation
The Norwegian EPD Foundation
Publisher:
Declaration number: NEPD-2024-895-EN
Registration number: NEPD-2024-895-EN
ECO Platform reference number: -
Issue date: 23.01.2020
Valid to: 23.01.2025
webertherm 261 putsbruk EF
Saint-Gobain Sweden AB, Weber
www.epd-norge.no
General information
Product: Owner of the declaration:
webertherm 261 putsbruk EF Saint-Gobain Sweden AB, Weber
Contact person: Anders Anderberg
Phone: +46 8 625 6105
e-mail: anders.anderberg@weber.se
Program operator: Manufacturer:
The Norwegian EPD Foundation Saint-Gobain Sweden AB, Weber
Pb. 5250 Majorstuen, 0303 Oslo
Phone: +47 97722020
e-mail: post@epd-norge.no
Declaration number: Place of production:
NEPD-2024-895-EN Saint-Gobain Sweden AB, Weber, Riksten
ECO Platform reference number: Management system:
ISO 9001, ISO 14001
This declaration is based on Product Category Rules: Organisation no:
CEN Standard EN 15804:2012+A1:2013 serves as core PCR. SE-556241-2592
Requirements on the EPD for Mineral factory-made mortar.
Statement of liability: Issue date: 23.01.2020
The owner of the declaration shall be liable for the underlying
information and evidence. EPD Norway shall not be liable with Valid to: 23.01.2025
respect to manufacturer information, life cycle assessment data and
evidences.
Declared unit: Year of study:
1 kg webertherm 261 putsbruk EF 2018
Declared unit with option: Comparability:
EPD of construction products may not be comparable if they not
A1,A2,A3,A4
comply with EN 15804 and seen in a building context.
Functional unit: Author of the Life Cycle Assessment:
The declaration is developed using eEPD v3.0 from LCA.no
Approval:
Company specific data are:
Collected/registered by: Charlotte Karlsson
Internal verification by: Helene Wallgren
Verification: Approved:
Independent verification of data, other environmental information and
the declaration according to ISO14025:2010, § 8.1.3 and § 8.1.4
External
Third party verifier:
Sign Sign
Senior Research Scientist, Anne Rønning
(Independent verifier approved by EPD Norway)
Product
Product description: Technical data:
webertherm 261 putsbruk EF is a factory-made fiber-reinforced dry mortar webertherm 261 putsbruk EF is tested and approved according to EN 998-
based on lime and cement with natural sand as aggregates. When mixed 1 and ETA SP 105 Fire.
with water, it is a ready-to-use render for indor and outdoor use.
webertherm 261 putsbruk EF is a hydrofobic render specially designed for Mortar category: CS III.
use in Serpomin EF facade systems and Serpovent G2. webertherm 261
putsbruk EF can also be used on both Exclay,bricks and Concrete as well For further information, see www.se.weber/
as previously renderd facades. webertherm 261 putsbruk EF is applied in
Market:
two layers, the first layer (> 6mm), and the second layer around 2-3 mm.
The render is sprayable and pumpable in a 60m hose. Sweden and Denmark
Reference service life, product
webertherm 261 putsbruk EF can be delivered in closed silos of 10 tons
with a flow mixer to avoid dust. The reference service life of the product is similar to the service life of the
building.
Product specification
Reference service life, building
50 years.
Materials %
Binder 10-30
Aggregate 60-90
Filler 5-10
Additives <5
Packaging <0,2
LCA: Calculation rules
Declared unit: Allocation:
The allocation is made in accordance with the provisions of EN 15804.
1 kg webertherm 261 putsbruk EF
Incoming energy and water and waste production in-house is allocated
Cut-off criteria: equally among all products through mass allocation. Effects of primary
All major raw materials and all the essential energy is included. The production of recycled materials is allocated to the main product in which
production processes for raw materials and energy flows with very small the material was used. The recycling process and transportation of the
amounts (less than 1%) are not included. These cut-off criteria do not material is allocated to this analysis.
apply for hazardous materials and substances.
Data quality:
Specific data for the product composition are provided by the manufacturer. They represent the production of the declared product and were collected
for EPD development in the year of study. Background data is based on registered EPDs according to EN 15804, Ostfold Research databases,
ecoinvent and other LCA databases. The data quality of the raw materials in A1 is presented in the table below.
Materials Source Data quality Year
Cement Supplier EPD 2014
Additives ecoinvent 3.4 Database 2017
Aggregate ecoinvent 3.4 Database 2017
Filler ecoinvent 3.4 Database 2017
Packaging ecoinvent 3.4 Database 2017
Packaging Modified ecoinvent 3.4 Database 2017
SC 99 Owner of EPD Database
SC 354 Owner of EPD Database 2018
SC 425 Owner of EPD Database 2019
System boundary:
"All processes from raw material extraction to product from the factory gate are included in the analysis (A1-A3). In addition, transportation to a central
warehouse placed in accordance with guidelines issued by the EPD Norway (A4) is included.
The flow chart below illustrates the system boundaries for the A1 to A3 part of the analysis."
Additional technical information:
webertherm 261 putsbruk EF is a render in the ventilated Serpovent G2 , Serpovent G2 has been verified for fire according to SP 105 Fire.
The remaining powder is classified as hazardous waste. Cured material is inactive and not classified as hazardous waste and may be disposed as
construction waste to disposal or recycling.
The packaging properly emptied is not classified as hazardous waste.
LCA: Scenarios and additional technical information
The following information describe the scenarios in the different modules of the EPD.
Transport from production place to user (A4)
Capacity
Fuel/Energy
Type utilisation (incl. Type of vehicle Distance km Unit Value (l/t)
consumption
return) %
Truck, lorry over
Truck 55,0 % 32 tonnes, EURO 152 0,022823 l/tkm 3,47
5
Railway l/tkm
Boat l/tkm
Other Transportation l/tkm
LCA: Results
System boundaries (X=included, MND=module not declared, MNR=module not relevant)
Construction Beyond the
Product stage installation User stage End of life stage . system
stage bondaries
A1 A2 A3 A4 A5 B1 B2 B3 B4 B5 B6 B7 C1 C2 C3 C4 . D
X X X X MND MND MND MND MND MND MND MND MND MND MND MND . MND
Environmental impact
Parameter Unit A1 A2 A3 A4
GWP kg CO 2 -eq 2,05E-01 1,48E-02 2,02E-02 1,33E-02
ODP kg CFC11 -eq 6,37E-09 2,27E-09 4,16E-09 2,58E-09
POCP kg C 2H 4-eq 4,32E-05 2,43E-06 6,18E-06 2,14E-06
AP kg SO 2 -eq 4,66E-04 5,00E-05 1,11E-04 4,31E-05
EP kg PO3- -eq 1,33E-04 8,52E-06 2,45E-05 7,23E-06
4
ADPM kg Sb -eq 5,45E-07 4,36E-08 1,97E-08 2,99E-08
ADPE MJ 2,58E+00 2,24E-01 3,23E-01 2,08E-01
GWP Global warming potential; ODP Depletion potential of the stratospheric ozone layer; POCP Formation potential of tropospheric photochemical
oxidants; AP Acidification potential of land and water; EP Eutrophication potential; ADPM Abiotic depletion potential for non fossil resources; ADPE
Abiotic depletion potential for fossil resources
Reading example: 9,0 E-03 = 9,0*10-3 = 0,009
*INA Indicator Not Assessed
waR slairetam tropsnarT
gnirutcafunaM
tropsnarT ylbmessA esU ecnanetniaM riapeR tnemecalpeR
tnemhsibrufeR
lanoitarepO ygrene esu lanoitarepO esu retaw -eD noitcurtsnoc noitilomed tropsnarT etsaW gnissecorp lasopsiD
-yrevoceR-esueR
-gnilcyceR laitnetop
Resource use
Parameter Unit A1 A2 A3 A4
RPEE MJ 3,52E-01 3,32E-03 2,63E-01 3,76E-03
RPEM MJ 1,02E-01 0,00E+00 0,00E+00 0,00E+00
TPE MJ 4,54E-01 3,32E-03 2,63E-01 3,76E-03
NRPE MJ 2,85E+00 2,30E-01 3,25E-01 2,14E-01
NRPM MJ 9,54E-02 0,00E+00 0,00E+00 0,00E+00
TRPE MJ 2,95E+00 2,30E-01 3,25E-01 2,14E-01
SM kg 8,71E-04 0,00E+00 0,00E+00 0,00E+00
RSF MJ 7,58E-02 0,00E+00 0,00E+00 0,00E+00
NRSF MJ 1,04E-01 0,00E+00 0,00E+00 0,00E+00
W m3 2,72E-03 4,66E-05 4,04E-05 5,05E-05
RPEE Renewable primary energy resources used as energy carrier; RPEM Renewable primary energy resources used as raw materials; TPE Total use
of renewable primary energy resources; NRPE Non renewable primary energy resources used as energy carrier; NRPM Non renewable primary energy
resources used as materials; TRPE Total use of non renewable primary energy resources; SM Use of secondary materials; RSF Use of renewable
secondary fuels; NRSF Use of non renewable secondary fuels; W Use of net fresh water
Reading example: 9,0 E-03 = 9,0*10-3 = 0,009
*INA Indicator Not Assessed
End of life - Waste
Parameter Unit A1 A2 A3 A4
HW kg 1,76E-06 1,37E-07 2,28E-05 1,14E-07
NHW kg 1,99E-02 1,31E-02 6,81E-02 1,95E-02
RW kg INA* INA* INA* INA*
HW Hazardous waste disposed; NHW Non hazardous waste disposed; RW Radioactive waste disposed
Reading example: 9,0 E-03 = 9,0*10-3 = 0,009
*INA Indicator Not Assessed
End of life - Output flow
Parameter Unit A1 A2 A3 A4
CR kg 0,00E+00 0,00E+00 0,00E+00 0,00E+00
MR kg 7,84E-08 0,00E+00 3,68E-04 0,00E+00
MER kg 3,21E-06 0,00E+00 1,55E-03 0,00E+00
EEE MJ INA* INA* INA* INA*
ETE MJ INA* INA* INA* INA*
CR Components for reuse; MR Materials for recycling; MER Materials for energy recovery; EEE Exported electric energy; ETE Exported thermal
energy
Reading example: 9,0 E-03 = 9,0*10-3 = 0,009
*INA Indicator Not Assessed
NEPD-2024-895-EN webertherm 261 putsbruk EF 7 / 8
Additional Norwegian requirements
Greenhouse gas emissions from the use of electricity in the manufacturing phase
National production mix from import, low voltage (production of transmission lines, in addition to direct emissions and losses in grid) of applied
electricity for the manufacturing process (A3).
Electricity mix Data source Amount Unit
Renewable electricity with Guarantee of Origin from LOS (kWh) Modified ecoinvent 3.4 60,20 g CO2-ekv/kWh
Dangerous substances
The product contains no substances given by the REACH Candidate list or the Norwegian priority list. The product is classified as hazardous waste
(Avfallsforskriften, Annex III), see table.
Name CASNo Amount
Portand Cement 65997-15-1 10-20%
Indoor environment
The product has no impact on the indoor environment.
Bibliography
ISO 14025:2010 Environmental labels and declarations - Type III environmental declarations - Principles and procedures.
ISO 14044:2006 Environmental management - Life cycle assessment - Requirements and guidelines.
EN 15804:2012+A1:2013 Environmental product declaration - Core rules for the product category of construction products.
ISO 21930:2017 Sustainability in buildings and civil engineering works. Core rules for environmental product declarations of construction products.
ecoinvent v3, Allocation, cut-off by classification, Swiss Centre of Life Cycle Inventories.
Iversen et al., (2018) eEPD v3.0 - Background information for EPD generator system, LCA.no report number 04.18
Iversen et al., (2019) EPD generator for Saint-Gobain Weber and Scanspac - Background information and LCA data, LCA.no report number 05.18
NPCR Part A: Construction products and services. Ver. 1.0. April 2017, EPD-Norge.
NPCR 009 Part B for technical-chemical products. Ver. 1.0 June 2018, EPD-Norge.
Product Category Rules for Environmental Product Declarations: Institut Bauen und Umwelt e.V. (IBU): Requirements on the EPD for Mineral
factorymade
mortar.
Program operator and publisher Phone: +47 97722020
The Norwegian EPD Foundation
Post Box 5250 Majorstuen, 0303 Oslo e-mail: post@epd-norge.no
0303 Oslo Norway web: www.epd-norge.no
Owner of the declaration Phone: +46 8 625 6105
Saint-Gobain Sweden AB, Weber Fax:
Box 415 e-mail: anders.anderberg@weber.se
SE-19162 Sollentuna web: www.weber.se
Author of the Life Cycle Assessment Phone: +47 916 50 916
LCA.no AS Fax:
Dokka 1C e-mail: post@lca.no
1671 Kråkerøy web: www.lca.no
Developer of EPD generator Phone: +47 916 50 916
LCA.no AS
Dokka 1C e-mail: post@lca.no
1671 Kråkerøy web: www.lca.no
ver1 2015
ENVIRONMENTAL PRODUCT DECLARATION
in accordance with ISO 14025, ISO 21930 and EN 15804
Owner of the declaration: Saint-Gobain Sweden AB, Weber
Program operator: The Norwegian EPD Foundation
The Norwegian EPD Foundation
Publisher:
Declaration number: NEPD-2024-895-EN
Registration number: NEPD-2024-895-EN
ECO Platform reference number: -
Issue date: 23.01.2020
Valid to: 23.01.2025
webertherm 261 putsbruk EF
Saint-Gobain Sweden AB, Weber
www.epd-norge.no
General information
Product: Owner of the declaration:
webertherm 261 putsbruk EF Saint-Gobain Sweden AB, Weber
Contact person: Anders Anderberg
Phone: +46 8 625 6105
e-mail: anders.anderberg@weber.se
Program operator: Manufacturer:
The Norwegian EPD Foundation Saint-Gobain Sweden AB, Weber
Pb. 5250 Majorstuen, 0303 Oslo
Phone: +47 97722020
e-mail: post@epd-norge.no
Declaration number: Place of production:
NEPD-2024-895-EN Saint-Gobain Sweden AB, Weber, Riksten
ECO Platform reference number: Management system:
ISO 9001, ISO 14001
This declaration is based on Product Category Rules: Organisation no:
CEN Standard EN 15804:2012+A1:2013 serves as core PCR. SE-556241-2592
Requirements on the EPD for Mineral factory-made mortar.
Statement of liability: Issue date: 23.01.2020
The owner of the declaration shall be liable for the underlying
information and evidence. EPD Norway shall not be liable with Valid to: 23.01.2025
respect to manufacturer information, life cycle assessment data and
evidences.
Declared unit: Year of study:
1 kg webertherm 261 putsbruk EF 2018
Declared unit with option: Comparability:
EPD of construction products may not be comparable if they not
A1,A2,A3,A4
comply with EN 15804 and seen in a building context.
Functional unit: Author of the Life Cycle Assessment:
The declaration is developed using eEPD v3.0 from LCA.no
Approval:
Company specific data are:
Collected/registered by: Charlotte Karlsson
Internal verification by: Helene Wallgren
Verification: Approved:
Independent verification of data, other environmental information and
the declaration according to ISO14025:2010, § 8.1.3 and § 8.1.4
External
Third party verifier:
Sign Sign
Senior Research Scientist, Anne Rønning
(Independent verifier approved by EPD Norway)
Product
Product description: Technical data:
webertherm 261 putsbruk EF is a factory-made fiber-reinforced dry mortar webertherm 261 putsbruk EF is tested and approved according to EN 998-
based on lime and cement with natural sand as aggregates. When mixed 1 and ETA SP 105 Fire.
with water, it is a ready-to-use render for indor and outdoor use.
webertherm 261 putsbruk EF is a hydrofobic render specially designed for Mortar category: CS III.
use in Serpomin EF facade systems and Serpovent G2. webertherm 261
putsbruk EF can also be used on both Exclay,bricks and Concrete as well For further information, see www.se.weber/
as previously renderd facades. webertherm 261 putsbruk EF is applied in
Market:
two layers, the first layer (> 6mm), and the second layer around 2-3 mm.
The render is sprayable and pumpable in a 60m hose. Sweden and Denmark
Reference service life, product
webertherm 261 putsbruk EF can be delivered in closed silos of 10 tons
with a flow mixer to avoid dust. The reference service life of the product is similar to the service life of the
building.
Product specification
Reference service life, building
50 years.
Materials %
Binder 10-30
Aggregate 60-90
Filler 5-10
Additives <5
Packaging <0,2
LCA: Calculation rules
Declared unit: Allocation:
The allocation is made in accordance with the provisions of EN 15804.
1 kg webertherm 261 putsbruk EF
Incoming energy and water and waste production in-house is allocated
Cut-off criteria: equally among all products through mass allocation. Effects of primary
All major raw materials and all the essential energy is included. The production of recycled materials is allocated to the main product in which
production processes for raw materials and energy flows with very small the material was used. The recycling process and transportation of the
amounts (less than 1%) are not included. These cut-off criteria do not material is allocated to this analysis.
apply for hazardous materials and substances.
Data quality:
Specific data for the product composition are provided by the manufacturer. They represent the production of the declared product and were collected
for EPD development in the year of study. Background data is based on registered EPDs according to EN 15804, Ostfold Research databases,
ecoinvent and other LCA databases. The data quality of the raw materials in A1 is presented in the table below.
Materials Source Data quality Year
Cement Supplier EPD 2014
Additives ecoinvent 3.4 Database 2017
Aggregate ecoinvent 3.4 Database 2017
Filler ecoinvent 3.4 Database 2017
Packaging ecoinvent 3.4 Database 2017
Packaging Modified ecoinvent 3.4 Database 2017
SC 99 Owner of EPD Database
SC 354 Owner of EPD Database 2018
SC 425 Owner of EPD Database 2019
System boundary:
"All processes from raw material extraction to product from the factory gate are included in the analysis (A1-A3). In addition, transportation to a central
warehouse placed in accordance with guidelines issued by the EPD Norway (A4) is included.
The flow chart below illustrates the system boundaries for the A1 to A3 part of the analysis."
Additional technical information:
webertherm 261 putsbruk EF is a render in the ventilated Serpovent G2 , Serpovent G2 has been verified for fire according to SP 105 Fire.
The remaining powder is classified as hazardous waste. Cured material is inactive and not classified as hazardous waste and may be disposed as
construction waste to disposal or recycling.
The packaging properly emptied is not classified as hazardous waste.
LCA: Scenarios and additional technical information
The following information describe the scenarios in the different modules of the EPD.
Transport from production place to user (A4)
Capacity
Fuel/Energy
Type utilisation (incl. Type of vehicle Distance km Unit Value (l/t)
consumption
return) %
Truck, lorry over
Truck 55,0 % 32 tonnes, EURO 152 0,022823 l/tkm 3,47
5
Railway l/tkm
Boat l/tkm
Other Transportation l/tkm
LCA: Results
System boundaries (X=included, MND=module not declared, MNR=module not relevant)
Construction Beyond the
Product stage installation User stage End of life stage . system
stage bondaries
A1 A2 A3 A4 A5 B1 B2 B3 B4 B5 B6 B7 C1 C2 C3 C4 . D
X X X X MND MND MND MND MND MND MND MND MND MND MND MND . MND
Environmental impact
Parameter Unit A1 A2 A3 A4
GWP kg CO 2 -eq 2,05E-01 1,48E-02 2,02E-02 1,33E-02
ODP kg CFC11 -eq 6,37E-09 2,27E-09 4,16E-09 2,58E-09
POCP kg C 2H 4-eq 4,32E-05 2,43E-06 6,18E-06 2,14E-06
AP kg SO 2 -eq 4,66E-04 5,00E-05 1,11E-04 4,31E-05
EP kg PO3- -eq 1,33E-04 8,52E-06 2,45E-05 7,23E-06
4
ADPM kg Sb -eq 5,45E-07 4,36E-08 1,97E-08 2,99E-08
ADPE MJ 2,58E+00 2,24E-01 3,23E-01 2,08E-01
GWP Global warming potential; ODP Depletion potential of the stratospheric ozone layer; POCP Formation potential of tropospheric photochemical
oxidants; AP Acidification potential of land and water; EP Eutrophication potential; ADPM Abiotic depletion potential for non fossil resources; ADPE
Abiotic depletion potential for fossil resources
Reading example: 9,0 E-03 = 9,0*10-3 = 0,009
*INA Indicator Not Assessed
waR slairetam tropsnarT
gnirutcafunaM
tropsnarT ylbmessA esU ecnanetniaM riapeR tnemecalpeR
tnemhsibrufeR
lanoitarepO ygrene esu lanoitarepO esu retaw -eD noitcurtsnoc noitilomed tropsnarT etsaW gnissecorp lasopsiD
-yrevoceR-esueR
-gnilcyceR laitnetop
Resource use
Parameter Unit A1 A2 A3 A4
RPEE MJ 3,52E-01 3,32E-03 2,63E-01 3,76E-03
RPEM MJ 1,02E-01 0,00E+00 0,00E+00 0,00E+00
TPE MJ 4,54E-01 3,32E-03 2,63E-01 3,76E-03
NRPE MJ 2,85E+00 2,30E-01 3,25E-01 2,14E-01
NRPM MJ 9,54E-02 0,00E+00 0,00E+00 0,00E+00
TRPE MJ 2,95E+00 2,30E-01 3,25E-01 2,14E-01
SM kg 8,71E-04 0,00E+00 0,00E+00 0,00E+00
RSF MJ 7,58E-02 0,00E+00 0,00E+00 0,00E+00
NRSF MJ 1,04E-01 0,00E+00 0,00E+00 0,00E+00
W m3 2,72E-03 4,66E-05 4,04E-05 5,05E-05
RPEE Renewable primary energy resources used as energy carrier; RPEM Renewable primary energy resources used as raw materials; TPE Total use
of renewable primary energy resources; NRPE Non renewable primary energy resources used as energy carrier; NRPM Non renewable primary energy
resources used as materials; TRPE Total use of non renewable primary energy resources; SM Use of secondary materials; RSF Use of renewable
secondary fuels; NRSF Use of non renewable secondary fuels; W Use of net fresh water
Reading example: 9,0 E-03 = 9,0*10-3 = 0,009
*INA Indicator Not Assessed
End of life - Waste
Parameter Unit A1 A2 A3 A4
HW kg 1,76E-06 1,37E-07 2,28E-05 1,14E-07
NHW kg 1,99E-02 1,31E-02 6,81E-02 1,95E-02
RW kg INA* INA* INA* INA*
HW Hazardous waste disposed; NHW Non hazardous waste disposed; RW Radioactive waste disposed
Reading example: 9,0 E-03 = 9,0*10-3 = 0,009
*INA Indicator Not Assessed
End of life - Output flow
Parameter Unit A1 A2 A3 A4
CR kg 0,00E+00 0,00E+00 0,00E+00 0,00E+00
MR kg 7,84E-08 0,00E+00 3,68E-04 0,00E+00
MER kg 3,21E-06 0,00E+00 1,55E-03 0,00E+00
EEE MJ INA* INA* INA* INA*
ETE MJ INA* INA* INA* INA*
CR Components for reuse; MR Materials for recycling; MER Materials for energy recovery; EEE Exported electric energy; ETE Exported thermal
energy
Reading example: 9,0 E-03 = 9,0*10-3 = 0,009
*INA Indicator Not Assessed
Additional Norwegian requirements
Greenhouse gas emissions from the use of electricity in the manufacturing phase
National production mix from import, low voltage (production of transmission lines, in addition to direct emissions and losses in grid) of applied
electricity for the manufacturing process (A3).
Electricity mix Data source Amount Unit
Renewable electricity with Guarantee of Origin from LOS (kWh) Modified ecoinvent 3.4 60,20 g CO2-ekv/kWh
Dangerous substances
The product contains no substances given by the REACH Candidate list or the Norwegian priority list. The product is classified as hazardous waste
(Avfallsforskriften, Annex III), see table.
Name CASNo Amount
Portand Cement 65997-15-1 10-20%
Indoor environment
The product has no impact on the indoor environment.
Bibliography
ISO 14025:2010 Environmental labels and declarations - Type III environmental declarations - Principles and procedures.
ISO 14044:2006 Environmental management - Life cycle assessment - Requirements and guidelines.
EN 15804:2012+A1:2013 Environmental product declaration - Core rules for the product category of construction products.
ISO 21930:2017 Sustainability in buildings and civil engineering works. Core rules for environmental product declarations of construction products.
ecoinvent v3, Allocation, cut-off by classification, Swiss Centre of Life Cycle Inventories.
Iversen et al., (2018) eEPD v3.0 - Background information for EPD generator system, LCA.no report number 04.18
Iversen et al., (2019) EPD generator for Saint-Gobain Weber and Scanspac - Background information and LCA data, LCA.no report number 05.18
NPCR Part A: Construction products and services. Ver. 1.0. April 2017, EPD-Norge.
NPCR 009 Part B for technical-chemical products. Ver. 1.0 June 2018, EPD-Norge.
Product Category Rules for Environmental Product Declarations: Institut Bauen und Umwelt e.V. (IBU): Requirements on the EPD for Mineral
factorymade
mortar.
Program operator and publisher Phone: +47 97722020
The Norwegian EPD Foundation
Post Box 5250 Majorstuen, 0303 Oslo e-mail: post@epd-norge.no
0303 Oslo Norway web: www.epd-norge.no
Owner of the declaration Phone: +46 8 625 6105
Saint-Gobain Sweden AB, Weber Fax:
Box 415 e-mail: anders.anderberg@weber.se
SE-19162 Sollentuna web: www.weber.se
Author of the Life Cycle Assessment Phone: +47 916 50 916
LCA.no AS Fax:
Dokka 1C e-mail: post@lca.no
1671 Kråkerøy web: www.lca.no
Developer of EPD generator Phone: +47 916 50 916
LCA.no AS
Dokka 1C e-mail: post@lca.no
1671 Kråkerøy web: www.lca.no
NEPD-2024-895-EN webertherm 261 putsbruk EF 8 / 8
