Environmental product declaration
In accordance with 14025 and EN15804+A2
weber LR+ Finishing plaster (weber LR+ Pintatasoite)
Owner of the declaration: Program operator:
Saint-Gobain Finland Oy The Norwegian EPD Foundation
Product: Declaration number:
weber LR+ Finishing plaster (weber LR+ Pintatasoite)
Registration number:
Declared unit:
1 kg Issue date:
This declaration is based on Product Category Rules: Valid to:
CEN Standard EN 15804:2012+A2:2019 serves as core
EPD Software:
PCR
The Norwegian EPD Foundation LCA.no EPD generator ID: 58446
NPCR 009:2021 Part B for Technical - Chemical products
for building and construction industry (Version 3.0)
1 / 11
General information
Product Owner of the declaration:
weber LR+ Finishing plaster (weber LR+ Pintatasoite) Saint-Gobain Finland Oy
Contact person: Anne Kaiser
Phone: +358400289933
e-mail: anne.kaiser@saint-gobain.com
Program operator: Manufacturer:
Post Box 5250 Majorstuen, 0303 Oslo, Norway Saint-Gobain Finland Oy
The Norwegian EPD Foundation P.O. Box 70
Phone: +47 23 08 80 00 Fi-00381 Helsinki, Finland
web: post@epd-norge.no
Declaration number: Place of production:
Saint-Gobain Weber Parainen
Parainen Premix plant, Kalkkitehtaantie
21600 Parainen, Finland
This declaration is based on Product Category Rules: Management system:
CEN Standard EN 15804:2012+A2:2019 serves as core PCR ISO 9001:2015, ISO 14001:2015 and OHSAS 18001:2007
NPCR 009:2021 Part B for Technical - Chemical products for building
and construction industry (Version 3.0)
Statement of liability: Organisation no:
The owner of the declaration shall be liable for the underlying FI09515553
information and evidence. EPD Norway shall not be liable with respect
to manufacturer information, life cycle assessment data and
evidences.​
Declared unit: Issue date:
1 kg weber LR+ Finishing plaster (weber LR+ Pintatasoite)
Declared unit with option: Valid to:
A1-A3,A4,A5,C1,C2,C3,C4,D
Year of study:
2022
Functional unit: Comparability:
not relevant EPD of construction products may not be comparable if they not
comply with EN 15804 and seen in a building context.
General information on verification of EPD from EPD tools: Development and verification of EPD:
Independent verification of data, other environmental information The declaration is created using EPD tool lca.tools ver EPD2022.03,
and the declaration according to ISO 14025:2010, § 8.1.3 and § 8.1.4. developed by LCA.no. The EPD tool is integrated in the company's
Individualthird party verification of each EPD is not required when the management system, and has been approved by EPD Norway.
EPD tool is i) integrated into the company's environmental
management system, ii) the procedures for use of the EPD tool are Developer of EPD: Päivi Pesu
approved by EPDNorway, and iii)the proccess is reviewed annualy. See
Reviewer of company-specific input data and EPD: Helene Løvkvist
Appendix G of EPD-Norway's General Programme Instructions for
Andersen
further information on EPD tools.
Verification of EPD tool: Approved:
Independent third party verification of the EPD tool, background data
and test-EPD in accordance with EPDNorway's procedures and
guidelines for verification and approval of EPD tools.
Third party verifier:
Anne Rønning, Norsus AS
(no signature required)
2 / 11
Product
Product description:
weber LR+ Finishing plaster is polymer-based, sprayable or manually spread wall levelling plaster for dry interiors. It is used in levelling the walls
and ceiling surfaces of dry interiors. The product is suitable for levelling stone material substrates and plasterboard and other board surfaces. The
product has good filling capacity and it is economical. Delivered in 20 kg bags. GTIN 6415910021023
Product specification
The composition of the product is described in the following table:
Materials Value Unit
Aggregate 95-99 %
Additives 1-5 %
Packaging, PE 0,005 kg
Packaging, pallet 0,021 kg
Technical data:
weber LR+ Finishing plaster is produced according to the requirements of EN 15824 (Finishing plaster for interior walls and ceilings).
Material consumption: approx. 1,2 kg/m²/1 mm layer
Recommended layer thickness: partial levelling up to 5 mm, total levelling 1-3 mm.
Recommended water content: approx. 6,4-7,2 l/20 kg.
More information: www.fi.weber/sisapinnat/hienot-seinatasoitteet/weber-lr-pintatasoite
Market:
Nordic and Baltic countries
Reference service life, product
The reference service life of the product is similar to the service life of the building.
Reference service life, building
60 years
LCA: Calculation rules
Declared unit:
1 kg weber LR+ Finishing plaster (weber LR+ Pintatasoite)
Cut-off criteria:
All major raw materials and all the essential energy is included. The production processes for raw materials and energy flows with very small
amounts (less than 1%) are not included. These cut-off criteria do not​ apply for hazardous materials and substances.
Allocation:
The allocation is made in accordance with the provisions of EN 15804. Incoming energy and water and waste production in-house is allocated
equally among all products through mass allocation. Effects of primary production of recycled materials is allocated to the main product in which
the material was used. The recycling process and transportation of the material is allocated to this analysis.
Data quality:
Specific data for the product composition are provided by the manufacturer. The data represent the production of the declared product and were
collected for EPD development in the year of study. Background data is based on EPDs according to EN 15804 and different LCA databases. The
data quality of the raw materials in A1 is presented in the table below.
Materials Source Data quality Year
Additives ecoinvent 3.6 Database 2019
Filler ecoinvent 3.6 Database 2019
Packaging ecoinvent 3.6 Database 2019
Packaging Modified ecoinvent 3.6 Database 2019
3 / 11
System boundaries (X=included, MND=module not declared, MNR=module not relevant)
Construction Beyond the system
Product stage Use stage End of life stage
installation stage boundaries
A1 A2 A3 A4 A5 B1 B2 B3 B4 B5 B6 B7 C1 C2 C3 C4 D
X X X X X MND MND MND MND MND MND MND X X X X X
System boundary:
All processes from raw materials extraction to product transportation to the building site, assembly as well as end of life stage and phases beyond
the system boundary (A1-A5, C1-C4, D) are included in the analysis.
The basic production process comprises of mixing raw materials together. Ready mixed product is then packed into bags for delivery. At assembly
phase, water is added according to the instructions and it is mixed. Stage B is not considered. Default waste treatment scenario from NPCR Part B
Technical - Chemical products for building and construction industry is applied: When building is demolished at the end-of-life 10% of the product
is collected for material recycling, and remaining 90% is disposed to landfill.
System boundaries (cradle-to-gate with options, modules A4-A5, C1-C4 and D) are illustrated in the picture below.
Additional technical information:
The LCA calculation has been made taking into account the fact that during the manufacturing process 100% renewable electricity is used. This
100% renewable electricity bought is evidenced by Guarantee of Origin certificates (GOs) from LOS, valid for the study year (2022) and after.
waR slairetam tropsnarT gnirutcafunaM tropsnarT ylbmessA e​sU ecnanetniaM riapeR tnemecalpeR tnemhsibrufeR lanoitarepO ygrene esu lanoitarepO esu retaw -eD noitcurtsnoc noitilomed tropsnarT etsaW gnissecorp lasopsiD -yrevoceR-esueR laitnetop-gnilcyceR
4 / 11
LCA: Scenarios and additional technical information
The following information describe the scenarios in the different modules of the EPD.
The results of stage A4 (transportation of product) in the table of this EPD refer to transportation in Finland (average distance 2022). This product
may also be delivered to the countries in the additional table "Transport from production place to user (A4)". In order to adapt the impact of
transportation to these countries, A4 figures from this EPD shall be multiplied by the multiplication factors below.
At assembly stage, it is assumed that mixing is done by electric mixer. Electricity mix used is that of Finland. Material loss is considered to be 0.
At end-of-life stage, it is assumed that 10% of demolition waste is collected and recycled, and 90% is disposed to landfill. Transport distance to
processing is estimated to be 30 km.
Capacity utilisation Value
Transport from production place to user (A4) Distance (km) Fuel/Energy Consumption Unit
(incl. return) % (Liter/tonne)
Truck, over 32 tonnes, EURO 5 (km) 53,3 % 203 0,023 l/tkm 4,67
Transport from production place to user (A4) Unit Value
Multiplication factor
Tullinge, Sweden (truck 60 km / ferry 324 km) 2,23
GWP/A4
Multiplication factor
Lillestrøm, Norway (truck 547 km / ferry 324 km) 4,63
GWP/A4
Multiplication factor
Karlslunde, Denmark (truck 709 km / ferry 324 km) 5,42
GWP/A4
Multiplication factor
Tallinn, Estonia (truck 183 km / ferry 88 km) 1,42
GWP/A4
Multiplication factor
Riga, Latvia (truck 491 km / ferry 88 km) 2,94
GWP/A4
Multiplication factor
Kaunas, Lithuania (truck 760 km / ferry 88 km) 4,27
GWP/A4
Assembly (A5) Unit Value
Electricity, Finland (kWh) kWh/DU 0,00
Waste, packaging, plastic (LDPE), to average
kg/DU 0,00
treatment (kg)
Waste, plastic packaging, mixture, to average
kg 0,00
treatment (kg)
Waste, wood packaging, average treatment (kg) kg 0,02
Water, tap water (L) kg/DU 0,36
De-construction demolition (C1) Unit Value
Demolition of building per kg product (kg) kg/DU 1,00
Capacity utilisation Value
Transport to waste processing (C2) Distance (km) Fuel/Energy Consumption Unit
(incl. return) % (Liter/tonne)
Truck, over 32 tonnes, EURO 5 (km) 53,3 % 30 0,023 l/tkm 0,69
Waste processing (C3) Unit Value
Waste treatment of product after demolition (kg) kg/DU 0,10
Disposal (C4) Unit Value
Disposal of product in landfill (kg) kg/DU 0,90
Benefits and loads beyond the system
Unit Value
boundaries (D)
Substitution of primary aggregates with crushed
kg/DU 0,10
recycled inert products (kg)
5 / 11
LCA: Results
The LCA results are presented below for the declared unit defined on page 2 of the EPD document.
Environmental impact
Indicator Unit A1-A3 A4 A5 C1 C2 C3 C4 D
GWP-total kg CO2 -eq 5,73E-02 1,85E-02 1,60E-03 4,00E-03 2,73E-03 7,20E-05 7,39E-03 -2,34E-04
GWP-fossil kg CO2 -eq 8,62E-02 1,84E-02 1,59E-03 4,00E-03 2,73E-03 7,10E-05 7,38E-03 -2,29E-04
GWP-biogenic kg CO2 -eq -2,89E-02 7,57E-06 6,40E-06 7,50E-07 1,12E-06 6,13E-07 8,62E-06 -4,57E-06
GWP-luluc kg CO2 -eq 7,93E-05 5,39E-06 6,17E-06 3,15E-07 7,96E-07 9,83E-08 1,81E-06 -1,55E-07
ODP kg CFC11 -eq 1,03E-08 4,26E-09 1,97E-10 8,64E-10 6,30E-10 1,40E-11 2,80E-09 -4,20E-11
AP mol H+ -eq 4,90E-04 7,76E-05 8,01E-06 4,19E-05 1,15E-05 5,75E-07 6,57E-05 -2,06E-06
EP-FreshWater kg P -eq 2,82E-06 1,41E-07 4,06E-08 1,46E-08 2,08E-08 4,49E-09 8,37E-08 -6,09E-09
EP-Marine kg N -eq 1,14E-04 2,33E-05 2,84E-06 1,85E-05 3,45E-06 1,68E-07 2,44E-05 -7,15E-07
EP-Terrestial mol N -eq 1,22E-03 2,58E-04 2,83E-05 2,00E-04 3,81E-05 1,94E-06 2,69E-04 -8,40E-06
POCP kg NMVOC -eq 3,91E-04 8,29E-05 7,46E-06 5,57E-05 1,23E-05 5,20E-07 7,71E-05 -2,22E-06
ADP-minerals&metals1 kg Sb -eq 1,06E-06 3,15E-07 1,88E-08 6,14E-09 4,66E-08 9,01E-10 6,65E-08 -2,03E-08
ADP-fossil1 MJ 1,97E+00 2,87E-01 2,63E-02 5,51E-02 4,24E-02 2,21E-03 2,03E-01 -3,87E-03
WDP1 m3 1,58E+00 2,20E-01 9,43E-01 1,17E-02 3,25E-02 2,43E-01 1,25E+00 -1,82E-01
GWP total Global Warming Potential total; GWP fossil Global Warming Potential fossil fuels ; GWP biogenic Global Warming Potential biogenic; GWP luluc Global W
Potential land use change; ODP Ozone Depletion; AP Acidification; EP freshwater Eutrophication aquatic freshwater; EP marine Eutrophication aquatic marine; EP
terrestrial Eutrophication terrestrial ;POCP Photochemical zone formation; ADPE Abiotic Depletion Potential minerals and metals; ADPf Abiotic Depletion Potential fossil
fuels; WDP Water Depletion Potential
"Reading example: 9,0 E-03 = 9,0*10-3 = 0,009"
*INA Indicator Not Assessed
1. The results of this environmental impact indicator shall be used with care as the uncertainties on these results are high or as there is limited experienced with the
indicator
Remarks to environmental impacts
6 / 11
Additional environmental impact indicators
Indicator Unit A1-A3 A4 A5 C1 C2 C3 C4 D
PM Disease incidence 4,43E-09 1,62E-09 8,00E-11 5,07E-09 2,40E-10 9,00E-12 1,40E-09 -4,40E-11
IRP2 kgBq U235 -eq 3,83E-03 1,25E-03 4,39E-04 2,40E-04 1,85E-04 3,70E-05 9,27E-04 -3,55E-05
ETP-fw1 CTUe 3,32E+00 2,10E-01 2,25E-02 3,01E-02 3,10E-02 1,56E-03 1,11E-01 -3,99E-03
HTP-c1 CTUh 4,60E-11 0,00E+00 1,00E-12 1,00E-12 0,00E+00 0,00E+00 5,00E-12 0,00E+00
HTP-nc1 CTUh 9,47E-10 2,03E-10 5,60E-11 2,80E-11 3,00E-11 1,00E-12 8,00E-11 -5,00E-12
SQP1 dimensionless 4,60E+00 3,29E-01 1,68E-02 6,69E-03 4,86E-02 1,25E-03 7,82E-01 8,79E-03
PM Particulate Matter emissions; IRP Ionizing radiation – human health; ETP-fw Eco toxicity – freshwater; HTP-c Human toxicity – cancer effects; HTP-nc Human
toxicity – non cancer effects; SQP Soil Quality (dimensionless)
"Reading example: 9,0 E-03 = 9,0*10-3 = 0,009"
*INA Indicator Not Assessed
1. The results of this environmental impact indicator shall be used with care as the uncertainties on these results are high or as there is limited experienced with the
indicator
2. This impact category deals mainly with the eventual impact of low dose ionizing radiation on human health of the nuclear fuel cycle. It does not consider effects due
to possible nuclear accidents, occupational exposure nor due to radioactive waste disposal in underground facilities. Potential ionizing radiation from the soil, from
radon and from some construction materials is also not measured by this indicator.
7 / 11
Resource use
Indicator Unit A1-A3 A4 A5 C1 C2 C3 C4 D
PERE MJ 7,00E-01 3,61E-03 5,44E-03 3,00E-04 5,34E-04 1,14E-03 7,27E-03 -9,07E-04
PERM MJ 2,89E-01 0,00E+00 0,00E+00 0,00E+00 0,00E+00 0,00E+00 0,00E+00 0,00E+00
PERT MJ 9,89E-01 3,61E-03 5,44E-03 3,00E-04 5,34E-04 1,14E-03 7,27E-03 -9,07E-04
PENRE MJ 1,31E+00 2,87E-01 2,68E-02 5,51E-02 4,24E-02 2,21E-03 2,03E-01 -4,09E-03
PENRM MJ 7,95E-01 0,00E+00 -5,31E-03 0,00E+00 0,00E+00 0,00E+00 0,00E+00 0,00E+00
PENRT MJ 2,10E+00 2,87E-01 2,15E-02 5,51E-02 4,24E-02 2,21E-03 2,03E-01 -4,09E-03
SM kg 6,18E-04 0,00E+00 4,06E-06 2,70E-05 0,00E+00 1,90E-06 8,81E-05 -7,83E-06
RSF MJ 3,76E-03 1,26E-04 8,61E-05 7,33E-06 1,87E-05 2,30E-05 1,51E-04 -1,85E-05
NRSF MJ 1,08E-03 4,23E-04 2,56E-04 -1,10E-04 6,26E-05 -1,42E-06 3,26E-04 -1,91E-05
FW m3 1,41E-03 3,27E-05 3,84E-04 2,83E-06 4,83E-06 3,78E-06 2,50E-04 -1,42E-04
PERE Use of renewable primary energy excluding renewable primary energy resources used as raw materials; PERM Use of renewable primary energy resources used as
raw materials; PERT Total use of renewable primary energy resources; PENRE Use of non renewable primary energy excluding non-renewable primary energy resources
used as raw materials; PENRM Use of non renewable primary energy resources used as raw materials; PENRT Total use of non renewable primary energy resources; SM
Use of secondary materials; RSF Use of renewable secondary fuels; NRSF Use of non renewable secondary fuels; FW Use of net fresh water
"Reading example: 9,0 E-03 = 9,0*10-3 = 0,009"
*INA Indicator Not Assessed
8 / 11
End of life - Waste
Indicator Unit A1-A3 A4 A5 C1 C2 C3 C4 D
HWD kg 1,08E-03 1,57E-05 2,17E-04 1,62E-06 2,32E-06 2,20E-07 1,43E-05 -9,34E-07
NHWD kg 1,92E-02 2,50E-02 2,78E-03 6,52E-05 3,69E-03 6,96E-06 9,01E-01 -2,83E-05
RWD kg 3,97E-06 1,96E-06 2,39E-07 3,82E-07 2,90E-07 2,33E-08 1,32E-06 -3,07E-08
HWD Hazardous waste disposed; NHWDNon-hazardous waste disposed; RWD Radioactive waste disposed;
"Reading example: 9,0 E-03 = 9,0*10-3 = 0,009"
*INA Indicator Not Assessed
End of life - Output flow
Indicator Unit A1-A3 A4 A5 C1 C2 C3 C4 D
CRU kg 0,00E+00 0,00E+00 0,00E+00 0,00E+00 0,00E+00 0,00E+00 0,00E+00 0,00E+00
MFR kg 1,56E-04 0,00E+00 2,44E-03 2,66E-05 0,00E+00 1,00E-01 8,03E-05 -1,83E-07
MER kg 1,31E-04 0,00E+00 5,44E-08 8,23E-08 0,00E+00 2,30E-07 1,51E-06 -6,86E-06
EEE MJ 2,52E-03 0,00E+00 1,45E-02 2,82E-07 0,00E+00 3,95E-07 1,25E-04 -1,66E-06
EET MJ 3,81E-02 0,00E+00 2,20E-01 4,27E-06 0,00E+00 5,97E-06 1,89E-03 -2,50E-05
CRU Components for re-use; MFR Materials for recycling; MER Materials for energy recovery; EEE Exported electrical energy; EET Exported energy Thermal
"Reading example: 9,0 E-03 = 9,0*10-3 = 0,009"
*INA Indicator Not Assessed
Biogenic Carbon Content
Indicator Unit At the factory gate
Biogenic carbon content in product kg C 0,00E+00
Biogenic carbon content in accompanying packaging kg C 8,61E-03
Note: 1 kg biogenic carbon is equivalent to 44/12 kg CO2
9 / 11
Additional Norwegian requirements
Greenhouse gas emissions from the use of electricity in the manufacturing phase
National production mix from import, low voltage (production of transmission lines, in addition to direct emissions and losses in grid) of applied
electricity for the manufacturing process (A3).
Electricity mix Data source Amount Unit
Renewable electricity Saint-Gobain, based on 100% hydro power, with Guarantee of Origin from LOS 2021 (kWh) ecoinvent 3.6 4,26 g CO2-eq/kWh
Dangerous substances
The product contains no substances given by the REACH Candidate list or the Norwegian priority list.
Indoor environment
weber LR+ Finishing plaster has M1 indoor air emission classification granted by The Finnish Building Information Foundation RTS
(https://cer.rts.fi/en/m1-emission-class-for-building-material/).
Additional Environmental Information
Environmental impact indicators EN 15804+A1 and NPCR Part A v2.0
Indicator Unit A1-A3 A4 A5 C1 C2 C3 C4 D
GWP kg CO2 -eq 9,77E-02 1,83E-02 1,69E-03 3,95E-03 2,70E-03 7,00E-05 7,23E-03 -2,45E-04
ODP kg CFC11 -eq 9,66E-09 3,45E-09 2,12E-10 6,86E-10 5,10E-10 1,70E-11 2,25E-09 -3,80E-11
POCP kg C2H4 -eq 3,00E-05 2,38E-06 2,90E-07 6,09E-07 3,52E-07 1,56E-08 1,70E-06 -5,11E-08
AP kg SO2 -eq 3,50E-04 3,68E-05 5,46E-06 5,84E-06 5,44E-06 2,63E-07 2,01E-05 -5,99E-07
EP kg PO43- -eq 4,90E-05 4,02E-06 1,29E-06 6,50E-07 5,94E-07 3,48E-08 2,37E-06 -7,02E-08
ADPM kg Sb -eq 1,06E-06 3,15E-07 1,88E-08 6,14E-09 4,66E-08 9,01E-10 6,65E-08 -2,03E-08
ADPE MJ 1,93E+00 2,82E-01 2,60E-02 5,47E-02 4,16E-02 8,47E-04 1,95E-01 -3,87E-03
GWPIOBC kg CO2 -eq 8,94E-02 1,85E-02 8,28E-04 5,37E+00 2,73E-03 0,00E+00 0,00E+00 -2,45E-04
GWP Global warming potential; ODP Depletion potential of the stratospheric ozone layer; POCP Formation potential of tropospheric photochemical oxidants; AP
Acidification potential of land and water; EP Eutrophication potential; ADPM Abiotic depletion potential for non fossil resources; ADPE Abiotic depletion​ potential for
fossil resources; GWP-IOBC/GHG Global warming potential calculated according to the principle of instantanious oxidation (except emissions and uptake of biogenic
carbon)
10 / 11
Bibliography
ISO 14025:2010 Environmental labels and declarations - Type III environmental declarations - Principles and procedures.
ISO 14044:2006 Environmental management - Life cycle assessment - Requirements and guidelines.
EN 15804:2012+A2:2019 Environmental product declaration - Core rules for the product category of construction products.
ISO 21930:2017 Sustainability in buildings and civil engineering works - Core rules for environmental product declarations of construction
products.
ecoinvent v3, Allocation, cut-off by classification, Swiss Centre of Life Cycle Inventories.
Iversen et al., (2021) eEPD v2021.09 Background information for EPD generator tool system verification, LCA.no Report number: 07.21
Iversen et al., (2019) EPD generator for Saint-Gobain Weber and Scanspac - Background information and LCA data, LCA.no report number 05.18
Iversen et al., (2020) EPD generator for Saint-Gobain Weber Nordics and Scanspac Background information for customer application,
and LCA data – Supplementary report for modules A5, C and D, LCA.no report number 04.20
NPCR Part A: Construction products and services. Ver. 2.0, 24.03.2021 EPD Norway.
NPCR 009 Part B for technical-chemical products. Ver. 2.0 October 2021, EPD-Norge.
Program operator and publisher Phone: +47 23 08 80 00
The Norwegian EPD Foundation e-mail: post@epd-norge.no
Post Box 5250 Majorstuen, 0303 Oslo, Norway web: www.epd-norge.no
Owner of the declaration: Phone: +358400289933
anne.kaiser@saint-
Saint-Gobain Finland Oy e-mail:
gobain.com
P.O. Box 70, Fi-00381 Helsinki web: www.saint-gobain.fi
Author of the Life Cycle Assessment Phone: +47 916 50 916
LCA.no AS e-mail: post@lca.no
Dokka 6B, 1671 web: www.lca.no
Developer of EPD generator Phone: +47 916 50 916
LCA.no AS e-mail: post@lca.no
Dokka 6B,1671 Kråkerøy web: www.lca.no
ECO Platform web: www.eco-platform.org
ECO Portal web: ECO Portal
11 / 11
