ver1 2015
ENVIRONMENTAL PRODUCT DECLARATION
in accordance with ISO 14025, ISO 21930 and EN 15804
Owner of the declaration: Saint-Gobain Sweden A B, Weber floor
Program operator: The Norwegian EP D Foundation
Publisher: The Norwegian EP D Foundation
Declaration number: NEPD-2302-1050-EN
Registration number: NEPD-2302-1050-EN
ECO Platform reference number: -
Issue date: 09.07.2020
Valid to: 09.07.2025
weberfloor 4610 industry top
Saint-Gobain Sweden AB, Weber floor
www.epd-norge.no
NEPD-2302-1050-EN weberfloor 4610 industry top 1 / 8
General information
Product: Owner of the declaration:
weberfloor 4610 industry top Saint-Gobain Sweden AB, Weber floor
Contact person: Anders Anderberg
Phone: +46 8 625 6105
e-mail: anders.anderberg@weber.se
Program operator: Manufacturer:
The Norwegian EP D Foundation Saint-Gobain Sweden AB, Weber floor
P b. 5250 Majorstuen, 0303 O slo
P hone: +47 23 08 80 00
e-mail: post@epd-norge.no
Declaration number: Place of production:
Saint-Gobain Sweden AB, Weber, Vingåker
NEPD-2302-1050-EN
ECO Platform reference number: Management system:
ISO 9001, ISO 14001
This declaration is based on Product Category Rules: Organisation no:
SE-556241-2592
CEN Standard EN 15804:2012+A1:2013 serves as core PCR.
Statement of liability: Issue date: 09.07.2020
The owner of the declaration shall be liable for the underlying
information and evidence. EPD Norway shall not be liable with Valid to: 09.07.2025
respect to manufacturer information, life cycle assessment data
and evidences.
Declared unit: Year of study:
1 kg weberfloor 4610 industry top 2019
Declared unit with option: Comparability:
EPD of construction products may not be comparable if they not
A1,A2,A3,A4,A5
comply with EN 15804 and seen in a building context.
Functional unit: Author of the Life Cycle Assessment:
The declaration is developed using eEPD v4.0 from LCA.no
Approval:
Company specific data are:
Collected/registered by: Thomas Flycht
Internal verification by: Helene Wallgren
Verification: Approved:
Independent verification of data, other environmental information
and the declaration according to ISO14025:2010, § 8.1.3 and §
8.1.4
External
Third party verifier:
Sign Sign
Senior Research Scientist, Anne Rønning
(Independent verifier approved by EPD Norway)
NEPD-2302-1050-EN weberfloor 4610 industry top 2 / 8
Product
Product description: Technical data:
weberfloor 4610 Industry Top is a pumpable, rapid hardening, self- weberfloor 4610 industry top is designed, produced and CE marked
levelling floor compound for use internally in buildings as a surface according to EN 13813
layer on industrial floors with medium or heavy rolling loading where
exceptional flatness is required, such as ware houses and high For further information, see www.se.weber/
racking storage areas. It is ready for traffic loading without further
Market:
finishing but may be coated with resin floorings.
Product specification Scandinavian countries
Reference service life, product
The composition of the product is described in the following table:
Materials % >50 years
Binder 15-40 Reference service life, building
Aggregate 30-60
>50 years
Filler 10-30
Additives 1-5
LCA: Calculation rules
Declared unit: Allocation:
The allocation is made in accordance with the provisions of EN
1 kg weberfloor 4610 industry top
15804. Incoming energy and water and waste production in-house
Cut-off criteria: is allocated equally among all products through mass allocation.
Effects of primary production of recycled materials is allocated to
All major raw materials and all the essential energy is included. The
the main product in which the material was used. The recycling
production processes for raw materials and energy flows with very
process and transportation of the material is allocated to this
small amounts (less than 1%) are not included. These cut-off
analysis.
criteria do not apply for hazardous materials and substances.
Data quality:
Specific data for the product composition are provided by the manufacturer. They represent the production of the declared product and were
collected for EPD development in the year of study. Background data is based on registered EPDs according to EN 15804, Ostfold
Research databases, ecoinvent and other LCA databases. The data quality of the raw materials in A1 is presented in the table below.
Materials Source Data quality Year
Cement Supplier EPD 2012
Binder EPD-BVG-20140073-IAG1-EN EPD 2014
Cement Supplier EPD 2014
Additives ecoinvent 3.4 Database 2017
Aggregate ecoinvent 3.4 Database 2017
Filler ecoinvent 3.4 Database 2017
Cement Supplier EPD 2018
NEPD-2302-1050-EN weberfloor 4610 industry top 3 / 8
System boundary:
All processes from raw material extraction to product transport to the construction site and assembly are included in the analysis (A1-A5).
The flow chart below illustrates the system boundaries for the A1 to A3 part of the analysis.
Additional technical information:
The consumption of the product is 1,7 kg / m² / mm.
The remaining powder and cured material may be disposed as construction waste to disposal or recycling.
NEPD-2302-1050-EN weberfloor 4610 industry top 4 / 8
LCA: Scenarios and additional technical information
The following information describe the scenarios in the different modules of the EPD.
Transport to market (A4) is calculated based on the default distance of 300 km from NPCR 013
Transport from production place to user (A4)
Capacity
Fuel/Energy
Type utilisation (incl. Type of vehicle Distance km Unit Value (l/t)
consumption
return) %
Truck, lorry over
Truck 55,0 % 32 tonnes, EURO 300 0,022823 l/tkm 6,85
5
Railway l/tkm
Boat l/tkm
Other Transportation l/tkm
Assembly (A5)
. Unit Value
Auxiliary kg
Water consumption m3 0,0002
Electricity consumption kWh 0,0021
Other energy carriers MJ
Material loss kg
Output materials from waste treatment kg 0,0000
Dust in the air kg
VOC emissions kg
NEPD-2302-1050-EN weberfloor 4610 industry top 5 / 8
LCA: Results
System boundaries (X=included, MND=module not declared, MNR=module not relevant)
Construction Beyond the
Product stage installation User stage End of life stage . system
stage bondaries
A1 A2 A3 A4 A5 B1 B2 B3 B4 B5 B6 B7 C1 C2 C3 C4 . D
X X X X X MND MND MND MND MND MND MND MND MND MND MND . MND
Environmental impact
Parameter Unit A1-A3 A4 A5
GWP kg CO 2 -eq 3,01E-01 2,62E-02 1,62E-04
ODP kg CFC11 -eq 2,85E-08 5,10E-09 1,06E-10
POCP kg C 2H 4-eq 7,31E-05 4,23E-06 4,66E-08
AP kg SO 2 -eq 1,27E-03 8,51E-05 8,67E-07
EP kg PO 3- -eq 1,79E-04 1,43E-05 1,65E-07
4
ADPM kg Sb -eq 3,14E-05 5,91E-08 1,43E-09
ADPE MJ 3,93E+00 4,11E-01 1,52E-03
GWP Global warming potential; ODP Depletion potential of the stratospheric ozone layer; POCP Formation potential of tropospheric photochemical
oxidants; AP Acidification potential of land and water; EP Eutrophication potential; ADPM Abiotic depletion potential for non fossil resources; ADPE
Abiotic depletion potential for fossil resources
Reading example: 9,0 E-03 = 9,0*10-3 = 0,009
*INA Indicator Not Assessed
waR slairetam tropsnarT gnirutcafunaM tropsnarT ylbmessA esU ecnanetniaM riapeR tnemecalpeR tnemhsibrufeR lanoitarepO ygrene esu lanoitarepO esu
retaw
-eD noitcurtsnoc noitilomed tropsnarT etsaW gnissecorp lasopsiD -yrevoceR-esueR -gnilcyceR laitnetop
NEPD-2302-1050-EN weberfloor 4610 industry top 6 / 8
Resource use
Parameter Unit A1-A3 A4 A5
RPEE MJ 4,01E-01 7,42E-03 5,94E-03
RPEM MJ 0,00E+00 0,00E+00 0,00E+00
TPE MJ 4,01E-01 7,42E-03 5,94E-03
NRPE MJ 4,58E+00 4,23E-01 1,43E-02
NRPM MJ 0,00E+00 0,00E+00 0,00E+00
TRPE MJ 4,58E+00 4,23E-01 1,43E-02
SM kg 7,64E-02 0,00E+00 0,00E+00
RSF MJ 1,86E-02 0,00E+00 5,60E-06
NRSF MJ 6,54E-01 0,00E+00 0,00E+00
W m3 6,46E-03 9,98E-05 2,37E-04
RPEE Renewable primary energy resources used as energy carrier; RPEM Renewable primary energy resources used as raw materials; TPE Total use
of renewable primary energy resources; NRPE Non renewable primary energy resources used as energy carrier; NRPM Non renewable primary energy
resources used as materials; TRPE Total use of non renewable primary energy resources; SM Use of secondary materials; RSF Use of renewable
secondary fuels; NRSF Use of non renewable secondary fuels; W Use of net fresh water
Reading example: 9,0 E-03 = 9,0*10-3 = 0,009
*INA Indicator Not Assessed
End of life - Waste
Parameter Unit A1-A3 A4 A5
HW kg 5,82E-05 2,25E-07 7,94E-09
NHW kg 6,40E-02 3,84E-02 1,39E-04
RW kg INA* INA* INA*
HW Hazardous waste disposed; NHW Non hazardous waste disposed; RW Radioactive waste disposed
Reading example: 9,0 E-03 = 9,0*10-3 = 0,009
*INA Indicator Not Assessed
End of life - Output flow
Parameter Unit A1-A3 A4 A5
CR kg 0,00E+00 0,00E+00 0,00E+00
MR kg 5,26E-05 0,00E+00 0,00E+00
MER kg 3,13E-04 0,00E+00 0,00E+00
EEE MJ INA* INA* INA*
ETE MJ INA* INA* INA*
CR Components for reuse; MR Materials for recycling; MER Materials for energy recovery; EEE Exported electric energy; ETE Exported thermal
energy
Reading example: 9,0 E-03 = 9,0*10-3 = 0,009
*INA Indicator Not Assessed
NEPD-2302-1050-EN weberfloor 4610 industry top 7 / 8
Additional Norwegian requirements
Greenhouse gas emissions from the use of electricity in the manufacturing phase
National production mix from import, low voltage (production of transmission lines, in addition to direct emissions and losses in grid) of
applied electricity for the manufacturing process (A3).
Electricity mix Data source Amount Unit
Renewable electricity with Guarantee of Origin from LOS (kWh) Modified ecoinvent 3.4 60,20 g CO2-ekv/kWh
Dangerous substances
The product contains no substances given by the REACH Candidate list or the Norwegian priority list.
Name CASNo Amount
Portland Cement CAS No 65997-15-1 2-5%
Indoor environment
The product meets the requirements for low emissions and odour (M1) by EN15251: 2007 Appendix E
Bibliography
ISO 14025:2010 Environmental labels and declarations - Type III environmental declarations - Principles and procedures.
ISO 14044:2006 Environmental management - Life cycle assessment - Requirements and guidelines.
EN 15804:2012+A1:2013 Environmental product declaration - Core rules for the product category of construction products.
ISO 21930:2017 Sustainability in buildings and civil engineering works. Core rules for environmental product declarations of construction
products.
ecoinvent v3, Allocation, cut-off by classification, Swiss Centre of Life Cycle Inventories.
Iversen et al., (2018) eEPD v3.0 - Background information for EPD generator system, LCA.no report number 04.18
Iversen et al., (2019) EPD generator for Saint-Gobain Weber and Scanspac - Background information and LCA data, LCA.no report number
05.18
NPCR Part A: Construction products and services. Ver. 1.0. April 2017, EPD-Norge.
NPCR 009 Part B for technical-chemical products. Ver. 1.0 June 2018, EPD-Norge.
Program operator and publisher Phone: +47 23 08 80 00
The Norwegian EPD Foundation
Post Box 5250 Majorstuen, 0303 Oslo e-mail: post@epd-norge.no
0303 Oslo Norway web: www.epd-norge.no
Owner of the declaration Phone: +46 8 625 6105
Saint-Gobain Sweden AB, Weber floor Fax:
Box 415 e-mail: anders.anderberg@weber.se
SE-19162 Sollentuna web: www.weber.se
Author of the Life Cycle Assessment Phone: +47 916 50 916
LCA.no AS Fax:
Dokka 1C e-mail: post@lca.no
1671 Kråkerøy web: www.lca.no
Developer of EPD generator Phone: +47 916 50 916
LCA.no AS
Dokka 1C e-mail: post@lca.no
1671 Kråkerøy web: www.lca.no
NEPD-2302-1050-EN weberfloor 4610 industry top 8 / 8
