ENVIRONMENTAL PRODUCT DECLARATION
as per ISO 14025 and EN 15804+A2
Owner of the Declaration SIGA Cover AG
Programme holder Institut Bauen und Umwelt e.V. (IBU)
Publisher Institut Bauen und Umwelt e.V. (IBU)
Declaration number EPD-SIG-20220186-CBA1-EN
Issue date 24.10.2022
Valid to 23.10.2027
Wetguard 200 SA
SIGA Cover AG
www.ibu-epd.com | https://epd-online.com
Umwelt Produktdeklaration Name des Herstellers – Name des Produkts
General Information
SIGA Cover AG Wetguard 200 SA
Programme holder Owner of the declaration
IBU – Institut Bauen und Umwelt e.V. SIGA Cover AG
Panoramastr. 1 Rütmattstrasse 7
10178 Berlin 6017 Ruswil
Germany Switzerland
Declaration number Declared product / declared unit
EPD-SIG-20220186-CBA1-EN Wetguard 200 SA / 1m²
This declaration is based on the product Scope:
category rules: This document applies to SIGA Wetguard 200 SA, a
False ceiling and underlay sheeting, 11.2017 fully self-adhesive temporary waterproof protection
(PCR checked and approved by the SVR) made of a slip-resistant non-woven membrane. It is
manufactured in Switzerland. The declared unit is 1 m2
with a unit weight of 260 g/m2. The LCA data were
Issue date
based on SIGA production data from the year 2020 by
24.10.2022
SIGA Manufacturing AG.
Valid to
The owner of the declaration shall be liable for the
23.10.2027
underlying information and evidence; the IBU shall not
be liable with respect to manufacturer information, life
cycle assessment data and evidences.
The EPD was created according to the specifications
of EN 15804+A2. In the following, the standard will be
simplified as EN 15804.
Verification
The standard EN 15804 serves as the core PCR
Independent verification of the declaration and data
according to ISO 14025:2010
Dipl. Ing. Hans Peters internally x externally
(chairman of Institut Bauen und Umwelt e.V.)
Dr. Alexander Röder Vito D'Incognito
(Managing Director Institut Bauen und Umwelt e.V.)) (Independent verifier)
Product
Product description/Product definition Technical Data
SIGA Wetguard 200 SA is a self-adhesive membrane
for temporary waterproof protection of wooden
elements during the building phase. The non-woven Constructional data
with anti-slip functional layer is fully covered with SIGA Name Value Unit
high-performance adhesive. Length acc. to EN 1848-2 50 m
0,39 / 0,78
Width acc. to EN 1848-2 m
/ 1,56
For the placing on the market in the EU/EFTA (with Straightness acc. to EN 1848-2 - mm/10m
exception of Switzerland) the regulation (EU) No Grammage acc. to EN 1849-2 0.24 kg/m2
305/2011 (CPR) applies. The products need a Resistance to water penetration
W1 -
declaration of performance taking into consideration acc. to EN 1928 (class)
EN 13984:2013, Flexible sheets for waterproofing - Water vapor diffusion equivalent
Plastic and rubber vapour control layers - Definitions air layer thickness acc. to EN 3.5 m
and characteristics and the CE-marking. For the 1931
application and use the respective national provisions Maximum tensile force acc. to EN
apply. 12311-1 150 N/50mm
Elongation acc. to EN 12311-1 80 %
Application
Tear Resistance (nail) acc. to EN
The diffusion open, robust , translucent and non- 80 N/mm
12310-1
slippery membrane is suitable for use as moisture
Flexibility at low temperatures acc.
protection for timber elements during the construction -40 °C
to EN 1109
phase, in particular for the full bonding of timber floors.
2 Environmental Product Declaration SIGA – Wetguard 200 SA
This product contains substances listed in the
Performance data of the product in accordance with candidate list (date: 01.01.2022) exceeding 0.1
the declaration of performance with respect to its percentage by mass: no.
essential characteristics according to EN 13984.
Reference service life
Base materials/Ancillary materials When installed according to the user manual, the
service life of the products is equal to the service life of
Name Value Unit the building element, where the product is a part of
Adhesive Acrylic Polymer 30 - 50 % (e.g. wall, roof etc.). The Sustainable Building
Fleece Polypropylene (PP) 15 - 25 % Assessment System BNB specifies the service life of
Functional Layer Polyolefin the building elements, where the product is used, as
15 - 25 %
Copolymer equal to or more than 50 years. A reference service life
Release Liner Polypropylene (PP) 15 - 25 % according to ISO 15686 is not reported.
LCA: Calculation rules
Declared Unit Construction stage - Modules A4-A5
The declared unit is 1m2 of Wetguard 200 SA with a The construction process stage includes:
grammage of 318 g/m2.This product comes with a  Transport to the construction site (A4)
polypropylene (PP) release liner (surface weight of  Treatment of packaging material (A5)
0.058 kg/ m2) that is later removed when the product is
applied.
Hence, this is deducted from the applied product End-of-life stage– Modules C1-C4 and D
weight considered for the LCA calculations (treated as The end-of-life stage includes
packaging instead) making the surface weight of the  Manual dismantling (C1)
applied product: 260 g/m2.  Transport to EoL (C2)
 Thermal treatment (C3). No disposal or
Declared unit
landfill processes (C4)
Name Value Unit
 Reuse, recovery or recycling potential (D) -
Declared unit 1 m2
Grammage 0.26 kg/m2 beyond system boundary includes credits
from thermal treatment (C3) and packaging
treatment (A5)
System boundary
31% of the total electricity demand is covered by green
Type of EPD according to EN 15804: "cradle to gate
electricity (Photovoltaics). The rest is calculated using
with options, modules C1–C4, and module D". The
country specific residual grid mix.
following modules are declared: A1–A3, C, D and
additional modules: A4 + A5.
Comparability
Basically, a comparison or an evaluation of EPD data
Production stage - Modules A1-A3
is only possible if all the data sets to be compared
The product stage includes:
were created according to EN 15804 and the building
 Raw material supply (A1)
context, respectively the product-specific
 Transport to the manufacturer (A2) characteristics of performance, are taken into account.
 Manufacturing (A3), including provision of all
materials, products and energy, as well as Background database: GaBi content update package
2021.2
waste processing up to the end-of waste
state.
LCA: Scenarios and additional technical information
Characteristic product properties The following technical scenario information is required
Information on biogenic Carbon for the declared modules and optional for non-declared
modules. The following technical information is a basis
for the declared modules or can be used for
Information on describing the biogenic Carbon developing specific scenarios in the context of a
Content at factory gate building assessment. The values refer to the declared
Name Value Unit unit of 1 m2 Wetguard 200 SA product.
Biogenic carbon content in
0 kg C
product Transport to the building site (A4)
Biogenic carbon content in Name Value Unit
0.0139 kg C
accompanying packaging Litres of fuel 0.0005 l/100km
Transport distance 100 km
Capacity utilisation (including 61 %
3 Environmental Product Declaration SIGA – Wetguard 200 SA
empty runs)
Gross density of products
- kg/m3
transported
Capacity utilisation volume factor - -
Gross unit weight of products
0.260 kg/m²
transported
Installation into the building (A5)
Name Value Unit
Waste packaging (PE foil) to
0.000196 kg
incineration
Waste packaging (wood) to
0.0206 kg
incineration
Waste packaging (Cores carton)
0.0168 kg
to incineration
Waste packaging (PP release
0.058 kg
liner) to incineration
End of life (C1-C4)
For the End-of-Life stage, the product dismantling (C1)
is done manually without environmental burden (load
free).
The transport to End of Life (C2) is calculated with a
distance of 50 km (with 61% utilization).
The Waste processing scenario adopted (C3) is
thermal treatment of the Wetguard 200 SA product. Its
incineration results in benefits, beyond the system
boundary, for thermal energy and electricity under
European conditions.
Name Value Unit
Collected separately (Wetguard
0.26 kg
200 SA)
Energy recovery 0.26 kg
Reuse, recovery and/or recycling potentials (D),
relevant scenario information
Module D includes the credits of the thermal and
electrical energy generated in Modules A5 and C3 due
to the thermal treatment of packaging and product
waste (Wetguard 200 SA product).
Avoided burdens have been calculated by the
inversion of residual grid mix and thermal energy from
natural gas, using European datasets.
A waste incineration plant with R1-value > 0.6 is
assumed.
4 Environmental Product Declaration SIGA – Wetguard 200 SA
LCA: Results
The following tables display the environmental relevant results according to /EN 15804/ for 1 m2 Wetguard
200SA.
Disclaimer:EP-freshwater: This indicator has been calculated as “kg P eq” as required in the characterization
model (EUTREND model, Struijs et al., 2009b, as implemented in ReCiPe;
http://eplca.jrc.ec.europa.eu/LCDN/developerEF.xhtml).
DESCRIPTION OF THE SYSTEM BOUNDARY (X = INCLUDED IN LCA; ND = MODULE OR INDICATOR NOT
DECLARED; MNR = MODULE NOT RELEVANT)
BENEFITS AND
CONSTRUCTI LOADS
PRODUCT STAGE ON PROCESS USE STAGE END OF LIFE STAGE BEYOND THE
STAGE SYSTEM
BOUNDARIES
5 Environmental Product Declaration SIGA – Wetguard 200 SA
lairetam
waR
ylppus tropsnarT
gnirutcafunaM
eht
morf
tropsnarT
etis
eht
ot
etag
ylbmessA esU
ecnanetniaM
riapeR
tnemecalpeR tnemhsibrufeR
ygrene
lanoitarepO esu
retaw
lanoitarepO esu
noitcurtsnoc-eD
noitilomed tropsnarT
gnissecorp
etsaW
lasopsiD -esueR -yrevoceR -gnilcyceR laitnetop
A1 A2 A3 A4 A5 B1 B2 B3 B4 B5 B6 B7 C1 C2 C3 C4 D
X X X X X ND ND MNR MNR MNR ND ND X X X X X
RESULTS OF THE LCA - ENVIRONMENTAL IMPACT according to EN 15804+A2: 1 m² Wetguard 200 SA
Core Indicator Unit A1-A3 A4 A5 C1 C2 C3 C4 D
GWP-total [kg CO2-Eq.] 1.11E+0 2.16E-3 2.47E-1 0.00E+0 1.58E-3 6.51E-1 0.00E+0 -4.60E-1
GWP-fossil [kg CO2-Eq.] 1.16E+0 2.13E-3 1.83E-1 0.00E+0 1.56E-3 6.51E-1 0.00E+0 -4.57E-1
GWP-biogenic [kg CO2-Eq.] -4.54E-2 6.09E-6 6.31E-2 0.00E+0 4.45E-6 9.74E-5 0.00E+0 -2.29E-3
GWP-luluc [kg CO2-Eq.] 6.46E-4 1.75E-5 1.74E-6 0.00E+0 1.28E-5 2.48E-5 0.00E+0 -3.17E-4
ODP [kg CFC11-Eq.] 2.34E-13 2.73E-19 2.31E-17 0.00E+0 2.00E-19 2.00E-16 0.00E+0 -5.24E-15
AP [mol H+-Eq.] 1.65E-3 2.02E-6 3.01E-5 0.00E+0 1.48E-6 8.34E-5 0.00E+0 -5.99E-4
EP-freshwater [kg PO4-Eq.] 3.42E-6 6.35E-9 3.32E-9 0.00E+0 4.64E-9 9.48E-8 0.00E+0 -5.99E-7
EP-marine [kg N-Eq.] 4.80E-4 6.25E-7 7.95E-6 0.00E+0 4.57E-7 2.29E-5 0.00E+0 -1.70E-4
EP-terrestrial [mol N-Eq.] 5.07E-3 7.51E-6 1.40E-4 0.00E+0 5.49E-6 3.79E-4 0.00E+0 -1.82E-3
POCP [kg NMVOC-Eq.] 1.80E-3 1.74E-6 2.24E-5 0.00E+0 1.27E-6 6.56E-5 0.00E+0 -4.77E-4
ADPE [kg Sb-Eq.] 2.27E-7 1.63E-10 3.51E-10 0.00E+0 1.19E-10 2.90E-9 0.00E+0 -7.62E-8
ADPF [MJ] 3.13E+1 2.85E-2 3.80E-2 0.00E+0 2.08E-2 2.54E-1 0.00E+0 -7.94E+0
[m³ world-Eq
WDP 1.18E-1 1.86E-5 2.36E-2 0.00E+0 1.36E-5 6.33E-2 0.00E+0 -3.52E-2
deprived]
GWP = Global warming potential; ODP = Depletion potential of the stratospheric ozone layer; AP = Acidification potential of land and water; EP =
Caption Eutrophication potential; POCP = Formation potential of tropospheric ozone photochemical oxidants; ADPE = Abiotic depletion potential for non-
fossil resources; ADPF = Abiotic depletion potential for fossil resources; WDP = Water (user) deprivation potential
RESULTS OF THE LCA - INDICATORS TO DESCRIBE RESOURCE USE according to EN 15804+A2: 1 m²
Wetguard 200 SA
Indicator Unit A1-A3 A4 A5 C1 C2 C3 C4 D
PERE [MJ] 2.61E+0 1.59E-3 5.72E-1 0.00E+0 1.16E-3 5.52E-2 0.00E+0 -1.80E+0
PERM [MJ] 5.64E-1 0.00E+0 -5.64E-1 0.00E+0 0.00E+0 0.00E+0 0.00E+0 0.00E+0
PERT [MJ] 3.18E+0 1.59E-3 7.41E-3 0.00E+0 1.16E-3 5.52E-2 0.00E+0 -1.80E+0
PENRE [MJ] 2.01E+1 2.85E-2 2.71E+0 0.00E+0 2.08E-2 8.72E+0 0.00E+0 -7.94E+0
PENRM [MJ] 1.12E+1 0.00E+0 -2.68E+0 0.00E+0 0.00E+0 -8.47E+0 0.00E+0 0.00E+0
PENRT [MJ] 3.13E+1 2.85E-2 3.80E-2 0.00E+0 2.08E-2 2.54E-1 0.00E+0 -7.94E+0
SM [kg] 0.00E+0 0.00E+0 0.00E+0 0.00E+0 0.00E+0 0.00E+0 0.00E+0 0.00E+0
RSF [MJ] 0.00E+0 0.00E+0 0.00E+0 0.00E+0 0.00E+0 0.00E+0 0.00E+0 0.00E+0
NRSF [MJ] 0.00E+0 0.00E+0 0.00E+0 0.00E+0 0.00E+0 0.00E+0 0.00E+0 0.00E+0
FW [m³] 8.40E-3 1.82E-6 5.53E-4 0.00E+0 1.33E-6 1.50E-3 0.00E+0 -1.76E-3
PERE = Use of renewable primary energy excluding renewable primary energy resources used as raw materials; PERM = Use of
renewable primary energy resources used as raw materials; PERT = Total use of renewable primary energy resources; PENRE = Use of
non-renewable primary energy excluding non-renewable primary energy resources used as raw materials; PENRM = Use of non-
Caption
renewable primary energy resources used as raw materials; PENRT = Total use of non-renewable primary energy resources; SM = Use
of secondary material; RSF = Use of renewable secondary fuels; NRSF = Use of non-renewable secondary fuels; FW = Use of net fresh
water
RESULTS OF THE LCA – WASTE CATEGORIES AND OUTPUT FLOWS according to EN 15804+A2:
1 m² Wetguard 200 SA
Indicator Unit A1-A3 A4 A5 C1 C2 C3 C4 D
HWD [kg] 9.41E-9 1.44E-12 6.84E-12 0.00E+0 1.05E-12 4.56E-11 0.00E+0 -1.79E-9
NHWD [kg] 1.37E-2 4.24E-6 1.73E-3 0.00E+0 3.10E-6 6.29E-2 0.00E+0 -3.73E-3
RWD [kg] 6.16E-4 3.45E-8 2.10E-6 0.00E+0 2.52E-8 9.94E-6 0.00E+0 -5.79E-4
CRU [kg] 0.00E+0 0.00E+0 0.00E+0 0.00E+0 0.00E+0 0.00E+0 0.00E+0 0.00E+0
MFR [kg] 0.00E+0 0.00E+0 0.00E+0 0.00E+0 0.00E+0 0.00E+0 0.00E+0 0.00E+0
MER [kg] 0.00E+0 0.00E+0 0.00E+0 0.00E+0 0.00E+0 0.00E+0 0.00E+0 0.00E+0
EEE [MJ] 5.61E-2 0.00E+0 4.79E-1 0.00E+0 0.00E+0 1.44E+0 0.00E+0 0.00E+0
EET [MJ] 1.06E-1 0.00E+0 8.53E-1 0.00E+0 0.00E+0 2.60E+0 0.00E+0 0.00E+0
HWD = Hazardous waste disposed; NHWD = Non-hazardous waste disposed; RWD = Radioactive waste disposed; CRU = Components
Caption for re-use; MFR = Materials for recycling; MER = Materials for energy recovery; EEE = Exported electrical energy; EET = Exported
thermal energy
RESULTS OF THE LCA – additional impact categories according to EN 15804+A2-optional:
1 m² Wetguard 200 SA
Indicator Unit A1-A3 A4 A5 C1 C2 C3 C4 D
[Disease
PM 1.64E-8 1.23E-11 1.70E-10 0.00E+0 9.03E-12 1.18E-9 0.00E+0 -5.15E-9
Incidence]
[kBq U235-
IRP 7.09E-2 4.94E-6 3.32E-4 0.00E+0 3.61E-6 1.30E-3 0.00E+0 -9.50E-2
Eq.]
ETP-fw [CTUe] 1.38E+1 2.06E-2 1.71E-2 0.00E+0 1.50E-2 2.08E-1 0.00E+0 -1.67E+0
HTP-c [CTUh] 3.64E-10 4.15E-13 1.60E-12 0.00E+0 3.04E-13 1.02E-11 0.00E+0 -7.57E-11
HTP-nc [CTUh] 1.82E-8 2.14E-11 5.37E-11 0.00E+0 1.57E-11 1.10E-9 0.00E+0 -2.99E-9
SQP [-] 7.62E+0 9.78E-3 1.04E-2 0.00E+0 7.15E-3 6.19E-2 0.00E+0 -1.23E+0
PM = Potential incidence of disease due to PM emissions; IR = Potential Human exposure efficiency relative to U235; ETP-fw = Potential
Caption comparative Toxic Unit for ecosystems; HTP-c = Potential comparative Toxic Unit for humans (cancerogenic); HTP-nc = Potential
comparative Toxic Unit for humans (not cancerogenic); SQP = Potential soil quality index
Disclaimer 1 – for the indicator “Potential Human exposure efficiency relative to U235”.
This impact category deals mainly with the eventual impact of low-dose ionizing
radiation on human health of the nuclear fuel cycle. It does not consider effects due to possible
nuclear accidents, occupational exposure or radioactive waste disposal in underground
facilities. Potential ionizing radiation from the soil, radon and from some construction materials is also not
measured by this indicator.
Disclaimer 2 – for the indicators “abiotic depletion potential for non-fossil resources”, “abiotic depletion potential
for fossil resources”, “water (user) deprivation potential, deprivation-weighted water consumption”, “potential
comparative toxic unit for ecosystems”, “potential comparative toxic unit for humans – cancerogenic”, “Potential
comparative toxic unit for humans - not cancerogenic”, “potential soil quality index”.
The results of this environmental impact indicator shall be used with care as the
uncertainties on these results are high as there is limited experience with the indicator.
References
Product related standards EN 12311-1:1999
Flexible sheets for waterproofing - Part 1: Bitumen
Assessment System for Sustainable Building sheets for roof waterproofing; Determination of tensile
2014-09 properties; German version EN 12311-1:1999
assessment_system_bnb.pdf (bnb-
nachhaltigesbauen.de) EN 13984:2013
Flexible sheets for waterproofing - Plastic and rubber
EN 1109:2013 vapour control layers - Definitions and characteristics;
Flexible sheets for waterproofing - Bitumen sheets for German version EN 13984:2013
roof waterproofing - Determination of flexibility at low
temperature; German version EN 1109:2013 ISO 15686-1:2011
Buildings and constructed assets - Service life
EN 1848-2:2001 planning - Part 1: General principles and framework
Flexible sheets for waterproofing - Determination of
length, width, straightness and flatness - Part 2: Plastic regulation (EU) No 305/2011
and rubber sheets for roof waterproofing; German EUR-Lex - 32011R0305 - EN - EUR-Lex (europa.eu)
version EN 1848-2:2001
the candidate list
EN 1928:2000 List of substances of very high concern for
Flexible sheets for waterproofing - Bitumen, plastic and authorisation - ECHA (europa.eu)
rubber sheets for roof waterproofing - Determination of
watertightness; German version EN 1928:2000
Standards
EN 1931:2001
Flexible sheets for waterproofing - Bitumen, plastic and EN 15804
rubber sheets for roof waterproofing - Determination of EN 15804:2019+A2, Sustainability of construction
water vapour transmission properties; German version works — Environmental Product Declarations — Core
EN 1931:2000 rules for the product category of construction products.
EN 12310-1:1999 ISO 14025
Flexible sheets for waterproofing - Part 1: Bitumen DIN EN ISO 14025:2011-10, Environmental labels and
sheets for roof waterproofing; determination of declarations — Type III environmental declarations —
resistance to tearing (nail shank); German version Principles and procedures.
EN 12310-1:1999
Further References
CPR
6 Environmental Product Declaration SIGA – Wetguard 200 SA
Regulation No. 305/2011: Construction Products Bauen und Umwelt e.V., 2021
Regulation of the European Parliament and of the www.ibu-epd.com
European Council, 2011.
PCR Part A
GaBi ts PCR - Part A: Calculation rules for the Life Cycle
GaBi ts dataset documentation for the software-system Assessment and Requirements on the Background
and databases, LBP, University of Stuttgart and Report, version 2.1, Institut Bauen und Umwelt e.V.,
thinkstep, Leinfelden-Echterdingen, 2021 2021, www.bau-umwelt.com
(https://www.gabi-software.com/support/gabi)
PCR Part B
IBU 2021 PCR – Part B: Requirements on the EPD for False
Institut Bauen und Umwelt e.V.: General Instructions ceiling and underlay sheeting, version 1.6, 2017,
for the EPD programme of Institut Bauen und Umwelt Institut Bauen und Umwelt e.V., www.bau-umwelt.com
e.V. EPD programme. Version 2.0. Berlin: Institut
7 Environmental Product Declaration SIGA – Wetguard 200 SA
Publisher
Institut Bauen und Umwelt e.V. Tel +49 (0)30 3087748- 0
Panoramastr. 1 Fax +49 (0)30 3087748- 29
10178 Berlin Mail info@ibu-epd.com
Germany Web www.ibu-epd.com
Programme holder
Institut Bauen und Umwelt e.V. Tel +49 (0)30 - 3087748- 0
Panoramastr 1 Fax +49 (0)30 – 3087748 - 29
10178 Berlin Mail info@ibu-epd.com
Germany Web www.ibu-epd.com
Author of the Life Cycle
Assessment Tel +49 711 341817-0
Sphera Solutions GmbH Fax +49 711 341817-25
Hauptstraße 111- 113 Mail info@sphera.com
70771 Leinfelden-Echterdingen Web www.sphera.com
Germany
Owner of the Declaration
SIGA Cover AG Tel 0041 41 499 69 69
Rüttmatstrasse 7 Fax 0041 41 496 62 63
6017 Ruswil Mail technik@siga.swiss
Switzerland Web www.siga.swiss
