ENVIRONMENTAL PRODUCT DECLARATION
as per ISO 14025 and EN 15804+A1
Owner of the Declaration ArcelorMittal Europe
Programme holder Institut Bauen und Umwelt e.V. (IBU)
Publisher Institut Bauen und Umwelt e.V. (IBU)
Declaration number EPD-ARC-20210132-CBB1-EN
Issue date 19.07.2021
Valid to 18.07.2026
XCarb™ Recycled and renewably produced
Structural steel sections and merchant bars
ArcelorMittal Europe
www.ibu-epd.com | https://epd-online.com
Umwelt Produktdeklaration Name des Herstellers – Name des Produkts
General Information
ArcelorMittal Europe XCarb™ Recycled and renewably
produced structural steel sections and
merchant bars
Programme holder Owner of the declaration
IBU – Institut Bauen und Umwelt e.V. ArcelorMittal Europe – Long Products
Panoramastr. 1 66, rue de Luxembourg
10178 Berlin L-4221 Esch-sur-Alzette
Germany Luxembourg
Declaration number Declared product / declared unit
EPD-ARC-20210132-CBB1-EN 1 metric tonne of XCarb™ Recycled and renewably
produced structural steel sections and merchant bars.
This declaration is based on the product Scope:
category rules: The declared unit is 1 metric tonne of
Structural steels, 11.2017 XCarb™ Recycled and renewably produced structural
(PCR checked and approved by the SVR) steel sections and merchant bars produced by
ArcelorMittal.
Issue date The Life Cycle Assessment is based on data collected
from the EAF plants involved in the production:
19.07.2021
Differdange & Esch-Belval (sites of Belval, Differdange
and Rodange) in Luxembourg; Bergara & Olaberria in
Valid to
Spain. The data used represent >95% of annual
18.07.2026 production with 2019 data for deliveries based on
Guarantee of Origins renewable electricity supply.
The owner of the declaration shall be liable for the
underlying information and evidence; the IBU shall not
be liable with respect to manufacturer information, life
cycle assessment data and evidences.
The EPD was created according to the specifications
of EN 15804+A1. In the following, the standard will be
simplified as EN 15804.
Verification
The standard EN 15804 serves as the core PCR
Independent verification of the declaration and data
according to ISO 14025:2010
Dipl. Ing. Hans Peters internally x externally
(chairman of Institut Bauen und Umwelt e.V.)
Dr. Alexander Röder Matthias Klingler
(Managing Director Institut Bauen und Umwelt e.V.)) (Independent verifier)
Product
Product description/Product definition For the application and use the respective national
This EPD applies to 1 metric tonne of provisions apply.
XCarb™ Recycled and renewably produced structural
steel sections and merchant bars in usual structural Application
steel grades for building industry based on a steel Structural steel sections and merchant bars are
production in Electric Arc Furnace with renewable intended for bolted, welded or otherwise connected
electricity supply with Guarantee of Origins. constructions of buildings, bridges and other
structures, as well as in composite steel and concrete
For the placing on the market of the product in the structures. For example:
EU/EFTA (with the exception of Switzerland)  Single-storey buildings (industrial and storage
Regulation (EU) No. 305/2011 (CPR) applies. The halls, etc.)
product needs a Declaration of Performance taking
 Multi-storey buildings (offices, residential,
into consideration EN 10025-1:2004, Hot rolled
shops, car parks, high rise, etc.)
products of structural steels – Part 1: General technical
delivery conditions/ and the CE-marking.  Bridges (railway, road, pedestrian, etc.)
2 Environmental Product Declaration ArcelorMittal – XCarb™ Recycled and renewably produced Structural steel sections
and merchant bars
Other structures (pylons, power plants, stadiums,  Product standards: EN 10025, ASTM A36-
convention centers, airports, stations, etc.) 14, ASTM A572-15, ASTM A588-
15, ASTM A709-13, ASTM A913/A913M-15
Technical Data
and ASTM A992-11.
This EPD is valid for XCarb™ Recycled and renewably
produced structural sections and merchant bars of  Fabrication standards: EN 1090-2, AISC 303-
various steel grades and different forms of delivery 10, AWSD1.1/D1.1M. The Standard EN 1090-
produced with a certified supply of renewable 2 applies to the execution of steel structures
electricity. and includes the requirements for factory
production control.
Performance data of the product in accordance with
the Declaration of Performance.
Additional information on structural steel and
Constructional data constructing with steel can be obtained from
Name Value Unit ArcelorMittal Sales Programme Sections & Merchant
Density 7850 kg/m3 Bars available at http://sections.arcelormittal.com.
Modulus of elasticity 210000 N/mm2
Coefficient of thermal expansion 12 10-6K-1 Base materials/Ancillary materials
The base material of XCarb™ Recycled and
Thermal conductivity 48 W/(mK)
renewably produced structural steel sections and
Melting point 1536 °C
merchant bars is iron. Alloying elements are added in
Shear modulus 81000 N/mm²
the form of ferroalloys or metals (most common
elements are Manganese and Silicon). Some small
quantities of other elements may be present in the
Performance data of the product in accordance with
steel.
the declaration of performance with respect to its
essential characteristics according to EN 10025-
No substances listed on the “Candidate List of
1:2004.
Substances of Very High Concern for Authorisation” by
the European Chemicals Agency EC 1907-2006 are
Specific information on dimension tolerances,
contained in the steel in declarable quantities.
constructional data, as well as mechanical and
chemical properties can be found in the relevant
This product contains substances listed in the
literature and/or the following standards:
candidate list (date: 22.2.2021) exceeding 0.1
 Design standards: The standards of EN
percentage by mass: no
1993 and EN 1994, respectively of
ANSI/AISC 360-16 apply to the design of Reference service life
steel structures and composite steel and A reference service life for XCarb™ Recycled and
concrete structures. They include the renewably produced structural steel sections and
requirements regarding serviceability, bearing merchant bars is not declared. These are construction
products with many different applications purposes.
capacity, durability and fire resistance of steel
The lifetime therefore will be limited by the service life
structures and composite steel and concrete
of the work.
structures.
LCA: Calculation rules
Declared Unit
The declaration refers to the functional unit of 1 metric System boundary
tonne of XCarb™ Recycled and renewably produced Type of the EPD: cradle-to-gate - with options. Module
structural steel sections and merchant bars as A1-A3, Module C3, Module C4 and Module D were
specified in Part B requirements on the EPD for considered.
structural steels.
Modules A1-A3 of the structural steel production
The final results reflect the weighted average per include the following:
production volume of plants: Differdange & Esch-  The provision of resources, additives, and
Belval (sites of Belval, Differdange and Rodange) in energy
Luxembourg; Bergara & Olaberria in Spain.
 Transport of resources and additives to the
production site
The background data are taken from GaBi ts
Documentation.  Production processes on-site including
energy, production of additives, disposal of
Declared unit production residues, and consideration of
Name Value Unit related emissions
Declared unit 1 t
 Recycling of production/manufacturing scrap.
Density 7850 kg/m3
Steel scrap is assumed to reach the end-of-
Conversion factor to 1 kg 0.001 -
waste status once is shredded and sorted,
3 Environmental Product Declaration ArcelorMittal – XCarb™ Recycled and renewably produced Structural steel sections
and merchant bars
thus becomes input to the product system in
the inventory. Module D refers to the end of life of the structural steel
sections and merchant bars, including reuse and
recycling.
Module C3 takes into account the sorting and
shredding of after-use steel to allow its orientation
Comparability
towards the recycling solutions. This process will also
Basically, a comparison or an evaluation of EPD data
produce losses due to efficiency that will be oriented
is only possible if all the data sets to be compared
towards landfill sites. A conservative value of 1%
were created according to EN 15804 and the building
landfill is then considered in C4.
context, respectively the product-specific
characteristics of performance, are taken into account.
Module C4 takes into account the waste disposal
including physical pre-treatment and management of
GaBi ts Software version 10.0.1.92 was used with
the disposal site. Steel is an inert material which does
GaBi Database 2021.1 to calculate this EPD.
not require any specific treatment on disposal site.
LCA: Scenarios and additional technical information
The end of life for average structural steel sections and
merchant bar products consists of 11% reuse, 88%
recycling and 1% landfill, with the corresponding
benefits and burdens. This is based on the European
Commission – Science Research Development Report
and on the Umweltbundesamt (German Environmental
Agency).
End of life (C1 - C4)
Name Value Unit
Reuse 110 kg
Recycling 880 kg
Landfilling 10 kg
Reuse, recovery and/or recycling potentials (D),
relevant scenario information
Name Value Unit
Reuse 11 %
Recycling 88 %
4 Environmental Product Declaration ArcelorMittal – XCarb™ Recycled and renewably produced Structural steel sections
and merchant bars
LCA: Results
DESCRIPTION OF THE SYSTEM BOUNDARY (X = INCLUDED IN LCA; MND = MODULE NOT DECLARED;
MNR = MODULE NOT RELEVANT)
BENEFITS AND
CONSTRUCTI LOADS
PRODUCT STAGE ON PROCESS USE STAGE END OF LIFE STAGE BEYOND THE
STAGE SYSTEM
BOUNDARIES
5 Environmental Product Declaration ArcelorMittal – XCarb™ Recycled and renewably produced Structural steel sections
and merchant bars
lairetam
waR
ylppus tropsnarT
gnirutcafunaM
eht
morf
tropsnarT
etis
eht
ot
etag
ylbmessA esU
ecnanetniaM
riapeR
tnemecalpeR tnemhsibrufeR
ygrene
lanoitarepO esu
retaw
lanoitarepO esu
noitcurtsnoc-eD
noitilomed tropsnarT
gnissecorp
etsaW
lasopsiD -esueR -yrevoceR -gnilcyceR laitnetop
A1 A2 A3 A4 A5 B1 B2 B3 B4 B5 B6 B7 C1 C2 C3 C4 D
X X X MND MND MND MND MNR MNR MNR MND MND MND MND X X X
RESULTS OF THE LCA - ENVIRONMENTAL IMPACT according to EN 15804+A1: 1 metric to of XCarb™
structural steel sections
Parameter Unit A1-A3 C3 C4 D
Global warming potential [kg CO2-Eq.] 3.33E+2 1.60E+0 1.43E-1 2.14E+2
Depletion potential of the stratospheric ozone layer [kg CFC11-Eq.] 4.84E-11 4.69E-14 7.83E-16 -4.74E-12
Acidification potential of land and water [kg SO2-Eq.] 7.46E-1 2.99E-3 8.57E-4 3.22E-1
Eutrophication potential [kg (PO4)3--Eq.] 7.51E-2 4.48E-4 9.72E-5 1.25E-2
Formation potential of tropospheric ozone photochemical
[kg ethene-Eq.] 8.27E-2 2.60E-4 6.58E-5 1.16E-1
oxidants
Abiotic depletion potential for non-fossil resources [kg Sb-Eq.] 4.04E-4 4.70E-7 1.44E-8 5.13E-4
Abiotic depletion potential for fossil resources [MJ] 3.81E+3 1.82E+1 1.95E+0 1.94E+3
RESULTS OF THE LCA - INDICATORS TO DESCRIBE RESOURCE USE according to EN 15804+A1: 1
metric to of XCarb™ structural steel sections
Parameter Unit A1-A3 C3 C4 D
Renewable primary energy as energy carrier [MJ] 7.53E+3 1.22E+1 2.70E-1 -1.04E+3
Renewable primary energy resources as material utilization [MJ] 0.00E+0 0.00E+0 0.00E+0 0.00E+0
Total use of renewable primary energy resources [MJ] 7.53E+3 1.22E+1 2.70E-1 -1.04E+3
Non-renewable primary energy as energy carrier [MJ] 4.00E+3 2.82E+1 2.01E+0 1.85E+3
Non-renewable primary energy as material utilization [MJ] 0.00E+0 0.00E+0 0.00E+0 0.00E+0
Total use of non-renewable primary energy resources [MJ] 4.00E+3 2.82E+1 2.01E+0 1.85E+3
Use of secondary material [kg] 1.16E+3 0.00E+0 0.00E+0 0.00E+0
Use of renewable secondary fuels [MJ] 0.00E+0 0.00E+0 0.00E+0 0.00E+0
Use of non-renewable secondary fuels [MJ] 0.00E+0 0.00E+0 0.00E+0 0.00E+0
Use of net fresh water [m³] 6.10E-1 1.18E-2 4.95E-4 1.09E+0
RESULTS OF THE LCA – WASTE CATEGORIES AND OUTPUT FLOWS according to EN 15804+A1:
1 metric to of XCarb™ structural steel sections
Parameter Unit A1-A3 C3 C4 D
Hazardous waste disposed [kg] 1.52E-6 7.00E-9 2.13E-10 -8.06E-7
Non-hazardous waste disposed [kg] 2.02E+0 1.89E-2 1.00E+1 -2.78E+1
Radioactive waste disposed [kg] 5.46E-2 3.89E-3 2.10E-5 -6.09E-3
Components for re-use [kg] 0.00E+0 1.10E+2 0.00E+0 0.00E+0
Materials for recycling [kg] 0.00E+0 8.80E+2 0.00E+0 0.00E+0
Materials for energy recovery [kg] 0.00E+0 0.00E+0 0.00E+0 0.00E+0
Exported electrical energy [MJ] 0.00E+0 0.00E+0 0.00E+0 0.00E+0
Exported thermal energy [MJ] 0.00E+0 0.00E+0 0.00E+0 0.00E+0
1163,1 kg scrap is used in the manufacturing of 1 tonne of XCarb™ Recycled and renewably produced structural
steel sections and merchant bars. After use, 880 kg steel is recycled, 110 kg is reused, and 10 kg is landfilled.
The potential environmental impact calculated for module D depends on the net amount of scrap left in the
system, which is 880-1163,1 + 127,94 = -155,17 kg.
This means that the system has a net negative output of 155,17 kg scrap, which carries a potential credit then,
module D shows an environmental burden.
References
EN 15804 PCR Part A
EN 15804+A1:2013, Sustainability of construction PCR - Part A: Calculation Rules for the Life Cycle
works — Environmental Product Declarations — Core Assessment and Requirements on the Project Report,
rules for the product category of construction products. Institut Bauen und Umwelt e.V., www.ibu-epd.com,
2021.
PCR 2017, Part B EN 1090-2
Requirements on the EPD for Structural steels - Institut EN 1090-2:2008, Execution of steel structures and
Bauen und Umwelt e.V., Berlin (pub.): From the range aluminum structures – Part 2: technical requirements
of Environmental Product for steel structures.
Declarations of Institute Construction and Environment
e.V. (IBU), 2017. AISC 303-10
AISC 303-10:2010, Code of Standard Practice for
GaBi ts Software Structural Steel Buildings and Bridges
GaBi ts Software and Databases for Life Cycle
Engineering. LBP, University of Stuttgart und PE AWSD1.1/D1.1M
International, 2013. AWSD1.1/D1.1M:2015, Structural Welding
Code–Steel.
GaBi ts Documentation
GaBi ts Documentation of the GaBi datasets for Life EN 1993
Cycle Engineering. LBP, Universitity of Stuttgart and EN 1993:2005, Eurocode 3: Design of steel structures.
PE International, 2011.
http://documentation.gabi-software.com EN 1994
EN 1994:2004, Eurocode 4: Design of composite steel
ASTM A36-14 and concrete structures.
ASTM A36-14:2014, Standard specification for carbon
structural steel. ANSI/AISC 360-16
ANSI/AISC 360-16:2016, Specification for Structural
ASTM A572-15 Steel Buildings.
ASTM A572-15:2015, Standard specification for
highstrength low-alloy Columbium-Vanadium structural Candidate list - REACH
quality steel. Regulation (EC) No 1907/2006 of the European
Parliament and of the Council on the Registration,
ASTM A588-15 Evaluation, Authorisation and Restriction
ASTM A588-15:2015, Standard specification for of Chemicals (REACH)
highstrength low-alloy structural steel, up to 50 ksi [345 https://echa.europa.eu/candidate-list-table
MPa] minimum yield point, with atmospheric corrosion
resistance. Sales Programme Sections & Merchant Bars
ArcelorMittal Europe - Long Products available at
ASTM A709-13 http://sections.arcelormittal.com.
ASTM A709-13:2013, Standard specification for
structural steel for bridges. Umweltbundesamt
Instrumente zur Wiederverwendung von Bauteilen und
ASTM A913/913M-15 hochwertigen Verwertung von Baustoffen. Texte
ASTM A913/913M-15:2015, Standard specification for 93/2015.
high-strength low-alloy steel shapes of structural http://www.umweltbundesamt.de/publikationen/instrum
quality, produced by quenching and self-tempering ente-zur-wiederverwendung-von-bauteilen
process (QST).
European Commission – Science Research
ASTM A992-11 Development Report
ASTM A992-11:2015, Standard specification for Life-Cycle Assessment (LCA) for steel construction.
structural steel shapes. Technical steel research, 2002.
EN 10025-1
EN 10025-1:2004, Hot rolled products of structural
steels. General technical delivery conditions.
6 Environmental Product Declaration ArcelorMittal – XCarb™ Recycled and renewably produced Structural steel sections
and merchant bars
Publisher
Institut Bauen und Umwelt e.V. Tel +49 (0)30 3087748- 0
Panoramastr. 1 Fax +49 (0)30 3087748- 29
10178 Berlin Mail info@ibu-epd.com
Germany Web www.ibu-epd.com
Programme holder
Institut Bauen und Umwelt e.V. Tel +49 (0)30 - 3087748- 0
Panoramastr 1 Fax +49 (0)30 – 3087748 - 29
10178 Berlin Mail info@ibu-epd.com
Germany Web www.ibu-epd.com
Author of the Life Cycle
Assessment Tel +352 5313 3010
ArcelorMittal Europe – Long Fax -
Products – Sections Mail
Rue de Luxembourg 66 sections.sales@arcelormittal.co
4221 Esch-sur-Alzette m
Luxembourg Web sections.arcelormittal.com
Owner of the Declaration
ArcelorMittal Europe – Long Tel +352 5313 3010
Products – Sections Fax -
Rue de Luxembourg 66 Mail
4221 Esch-sur-Alzette sections.sales@arcelormittal.co
Luxembourg m
Web sections.arcelormittal.com
