{"product_name":"XCarb\u00ae recycled and renewably produced organic coated steel coils Granite\u00ae and Estetic\u00ae ","epd_id":"EPD-ARC-20220319-CBA1-EN","compliance":["DIN EN 15804+A2","ISO 14025"],"producer_name":"ArcelorMittal Europe \u2013 Flat Products","environmental_impact":[{"parameter":"GWP-total","unit":"kg CO2-eq.","values":[{"value":"1,03E+03","module":"A1-A3","scenario":null},{"value":"4,35E+01","module":"C1","scenario":null},{"value":"2,13E+01","module":"C2","scenario":null},{"value":"1,53E+00","module":"C3","scenario":null},{"value":"2,90E-01","module":"C4","scenario":null},{"value":"-1,40E+02","module":"D","scenario":null}]},{"parameter":"GWP-fossil","unit":"kg CO2-eq.","values":[{"value":"1,03E+03","module":"A1-A3","scenario":null},{"value":"4,32E+01","module":"C1","scenario":null},{"value":"2,11E+01","module":"C2","scenario":null},{"value":"1,52E+00","module":"C3","scenario":null},{"value":"2,98E-01","module":"C4","scenario":null},{"value":"-1,40E+02","module":"D","scenario":null}]},{"parameter":"GWP-biogenic","unit":"kg CO2-eq.","values":[{"value":"0,00E+00","module":"A1-A3","scenario":null},{"value":"1,83E-03","module":"C1","scenario":null},{"value":"1,53E-02","module":"C2","scenario":null},{"value":"5,40E-03","module":"C3","scenario":null},{"value":"-8,84E-03","module":"C4","scenario":null},{"value":"2,24E-01","module":"D","scenario":null}]},{"parameter":"GWP-luluc","unit":"kg CO2-eq.","values":[{"value":"2,93E-01","module":"A1-A3","scenario":null},{"value":"2,82E-01","module":"C1","scenario":null},{"value":"1,45E-01","module":"C2","scenario":null},{"value":"9,36E-04","module":"C3","scenario":null},{"value":"5,51E-04","module":"C4","scenario":null},{"value":"-3,75E-02","module":"D","scenario":null}]},{"parameter":"ODP","unit":"kg CFC11-eq.","values":[{"value":"8,59E-08","module":"A1-A3","scenario":null},{"value":"1,33E-11","module":"C1","scenario":null},{"value":"2,12E-12","module":"C2","scenario":null},{"value":"1,99E-11","module":"C3","scenario":null},{"value":"7,01E-13","module":"C4","scenario":null},{"value":"3,88E-10","module":"D","scenario":null}]},{"parameter":"AP","unit":"mol H^(+)-eq.","values":[{"value":"3,07E+00","module":"A1-A3","scenario":null},{"value":"2,46E-01","module":"C1","scenario":null},{"value":"1,27E-01","module":"C2","scenario":null},{"value":"3,75E-03","module":"C3","scenario":null},{"value":"2,12E-03","module":"C4","scenario":null},{"value":"-3,84E-01","module":"D","scenario":null}]},{"parameter":"POCP","unit":"kg NMVOC-eq.","values":[{"value":"2,29E+00","module":"A1-A3","scenario":null},{"value":"2,31E-01","module":"C1","scenario":null},{"value":"1,20E-01","module":"C2","scenario":null},{"value":"2,82E-03","module":"C3","scenario":null},{"value":"1,64E-03","module":"C4","scenario":null},{"value":"-2,67E-01","module":"D","scenario":null}]},{"parameter":"ADPE","unit":"kg Sb-eq.","values":[{"value":"2,16E-01","module":"A1-A3","scenario":null},{"value":"4,45E-06","module":"C1","scenario":null},{"value":"2,17E-06","module":"C2","scenario":null},{"value":"3,84E-07","module":"C3","scenario":null},{"value":"3,06E-08","module":"C4","scenario":null},{"value":"3,08E-06","module":"D","scenario":null}]},{"parameter":"ADPF","unit":"MJ","values":[{"value":"1,39E+04","module":"A1-A3","scenario":null},{"value":"5,82E+02","module":"C1","scenario":null},{"value":"2,83E+02","module":"C2","scenario":null},{"value":"2,68E+01","module":"C3","scenario":null},{"value":"3,91E+00","module":"C4","scenario":null},{"value":"-1,04E+03","module":"D","scenario":null}]},{"parameter":"WDP","unit":"m^3 world-eq. deprived","values":[{"value":"2,20E+02","module":"A1-A3","scenario":null},{"value":"6,26E-01","module":"C1","scenario":null},{"value":"2,41E-01","module":"C2","scenario":null},{"value":"3,11E-01","module":"C3","scenario":null},{"value":"3,27E-02","module":"C4","scenario":null},{"value":"2,93E+00","module":"D","scenario":null}]},{"parameter":"EP-freshwater","unit":"kg PO4-eq.","values":[{"value":"2,96E-03","module":"A1-A3","scenario":null},{"value":"1,52E-04","module":"C1","scenario":null},{"value":"7,70E-05","module":"C2","scenario":null},{"value":"4,31E-06","module":"C3","scenario":null},{"value":"5,06E-07","module":"C4","scenario":null},{"value":"-2,50E-05","module":"D","scenario":null}]},{"parameter":"EP-marine","unit":"kg N-eq.","values":[{"value":"7,06E-01","module":"A1-A3","scenario":null},{"value":"1,19E-01","module":"C1","scenario":null},{"value":"6,20E-02","module":"C2","scenario":null},{"value":"1,03E-03","module":"C3","scenario":null},{"value":"5,41E-04","module":"C4","scenario":null},{"value":"-8,01E-02","module":"D","scenario":null}]},{"parameter":"EP-terrestrial","unit":"mol N-eq.","values":[{"value":"7,56E+00","module":"A1-A3","scenario":null},{"value":"1,32E+00","module":"C1","scenario":null},{"value":"6,87E-01","module":"C2","scenario":null},{"value":"1,10E-02","module":"C3","scenario":null},{"value":"5,94E-03","module":"C4","scenario":null},{"value":"-8,67E-01","module":"D","scenario":null}]}],"additional_environmental_impact":[{"parameter":"PM","unit":"Disease incidence","values":[{"value":null,"module":"A1-A3","scenario":null},{"value":null,"module":"C1","scenario":null},{"value":null,"module":"C2","scenario":null},{"value":null,"module":"C3","scenario":null},{"value":null,"module":"C4","scenario":null},{"value":null,"module":"D","scenario":null}]},{"parameter":"ETP-fw","unit":"CTUe","values":[{"value":null,"module":"A1-A3","scenario":null},{"value":null,"module":"C1","scenario":null},{"value":null,"module":"C2","scenario":null},{"value":null,"module":"C3","scenario":null},{"value":null,"module":"C4","scenario":null},{"value":null,"module":"D","scenario":null}]},{"parameter":"HTP-c","unit":"CTUh","values":[{"value":null,"module":"A1-A3","scenario":null},{"value":null,"module":"C1","scenario":null},{"value":null,"module":"C2","scenario":null},{"value":null,"module":"C3","scenario":null},{"value":null,"module":"C4","scenario":null},{"value":null,"module":"D","scenario":null}]},{"parameter":"HTP-nc","unit":"CTUh","values":[{"value":null,"module":"A1-A3","scenario":null},{"value":null,"module":"C1","scenario":null},{"value":null,"module":"C2","scenario":null},{"value":null,"module":"C3","scenario":null},{"value":null,"module":"C4","scenario":null},{"value":null,"module":"D","scenario":null}]},{"parameter":"SQP","unit":"SQP","values":[{"value":null,"module":"A1-A3","scenario":null},{"value":null,"module":"C1","scenario":null},{"value":null,"module":"C2","scenario":null},{"value":null,"module":"C3","scenario":null},{"value":null,"module":"C4","scenario":null},{"value":null,"module":"D","scenario":null}]}],"resource_use":[{"parameter":"PERE","unit":"MJ","values":[{"value":"2,06E+04","module":"A1-A3","scenario":null},{"value":"4,44E+01","module":"C1","scenario":null},{"value":"1,96E+01","module":"C2","scenario":null},{"value":"1,38E+01","module":"C3","scenario":null},{"value":"5,86E-01","module":"C4","scenario":null},{"value":"1,52E+02","module":"D","scenario":null}]},{"parameter":"PERM","unit":"MJ","values":[{"value":"6,00E+01","module":"A1-A3","scenario":null},{"value":"0,00E+00","module":"C1","scenario":null},{"value":"0,00E+00","module":"C2","scenario":null},{"value":"0,00E+00","module":"C3","scenario":null},{"value":"0,00E+00","module":"C4","scenario":null},{"value":"-2,00E-01","module":"D","scenario":null}]},{"parameter":"PERT","unit":"MJ","values":[{"value":"2,07E+04","module":"A1-A3","scenario":null},{"value":"4,44E+01","module":"C1","scenario":null},{"value":"1,96E+01","module":"C2","scenario":null},{"value":"1,38E+01","module":"C3","scenario":null},{"value":"5,86E-01","module":"C4","scenario":null},{"value":"1,51E+02","module":"D","scenario":null}]},{"parameter":"PENRE","unit":"MJ","values":[{"value":"1,39E+04","module":"A1-A3","scenario":null},{"value":"5,85E+02","module":"C1","scenario":null},{"value":"2,84E+02","module":"C2","scenario":null},{"value":"2,68E+01","module":"C3","scenario":null},{"value":"3,91E+00","module":"C4","scenario":null},{"value":"-1,05E+03","module":"D","scenario":null}]},{"parameter":"PENRM","unit":"MJ","values":[{"value":"4,00E+01","module":"A1-A3","scenario":null},{"value":"0,00E+00","module":"C1","scenario":null},{"value":"0,00E+00","module":"C2","scenario":null},{"value":"0,00E+00","module":"C3","scenario":null},{"value":"0,00E+00","module":"C4","scenario":null},{"value":"1,00E+00","module":"D","scenario":null}]},{"parameter":"PENRT","unit":"MJ","values":[{"value":"1,40E+04","module":"A1-A3","scenario":null},{"value":"5,85E+02","module":"C1","scenario":null},{"value":"2,84E+02","module":"C2","scenario":null},{"value":"2,68E+01","module":"C3","scenario":null},{"value":"3,91E+00","module":"C4","scenario":null},{"value":"-1,05E+03","module":"D","scenario":null}]},{"parameter":"SM","unit":"kg","values":[{"value":"9,09E+02","module":"A1-A3","scenario":null},{"value":"0,00E+00","module":"C1","scenario":null},{"value":"0,00E+00","module":"C2","scenario":null},{"value":"0,00E+00","module":"C3","scenario":null},{"value":"0,00E+00","module":"C4","scenario":null},{"value":"7,11E+01","module":"D","scenario":null}]},{"parameter":"RSF","unit":"MJ","values":[{"value":"0,00E+00","module":"A1-A3","scenario":null},{"value":"0,00E+00","module":"C1","scenario":null},{"value":"0,00E+00","module":"C2","scenario":null},{"value":"0,00E+00","module":"C3","scenario":null},{"value":"0,00E+00","module":"C4","scenario":null},{"value":"0,00E+00","module":"D","scenario":null}]},{"parameter":"NRSF","unit":"MJ","values":[{"value":"0,00E+00","module":"A1-A3","scenario":null},{"value":"0,00E+00","module":"C1","scenario":null},{"value":"0,00E+00","module":"C2","scenario":null},{"value":"0,00E+00","module":"C3","scenario":null},{"value":"0,00E+00","module":"C4","scenario":null},{"value":"0,00E+00","module":"D","scenario":null}]},{"parameter":"FW","unit":"m^3","values":[{"value":"5,44E+00","module":"A1-A3","scenario":null},{"value":"5,04E-02","module":"C1","scenario":null},{"value":"2,27E-02","module":"C2","scenario":null},{"value":"1,32E-02","module":"C3","scenario":null},{"value":"9,93E-04","module":"C4","scenario":null},{"value":"-9,10E-02","module":"D","scenario":null}]}],"end_of_life_waste":[{"parameter":"HWD","unit":"kg","values":[{"value":"3,75E-06","module":"A1-A3","scenario":null},{"value":"4,07E-09","module":"C1","scenario":null},{"value":"1,50E-09","module":"C2","scenario":null},{"value":"7,90E-08","module":"C3","scenario":null},{"value":"0,00E+00","module":"C4","scenario":null},{"value":"5,21E-08","module":"D","scenario":null}]},{"parameter":"NHWD","unit":"kg","values":[{"value":"2,25E+01","module":"A1-A3","scenario":null},{"value":"1,03E-01","module":"C1","scenario":null},{"value":"4,63E-02","module":"C2","scenario":null},{"value":"1,90E-02","module":"C3","scenario":null},{"value":"2,00E+01","module":"C4","scenario":null},{"value":"-1,99E+00","module":"D","scenario":null}]},{"parameter":"RWD","unit":"kg","values":[{"value":"5,48E-01","module":"A1-A3","scenario":null},{"value":"2,86E-03","module":"C1","scenario":null},{"value":"5,27E-04","module":"C2","scenario":null},{"value":"3,95E-03","module":"C3","scenario":null},{"value":"4,35E-05","module":"C4","scenario":null},{"value":"1,74E-02","module":"D","scenario":null}]}],"end_of_life_flow":[{"parameter":"CRU","unit":"kg","values":[{"value":"0,00E+00","module":"A1-A3","scenario":null},{"value":"0,00E+00","module":"C1","scenario":null},{"value":"0,00E+00","module":"C2","scenario":null},{"value":"0,00E+00","module":"C3","scenario":null},{"value":"0,00E+00","module":"C4","scenario":null},{"value":"0,00E+00","module":"D","scenario":null}]},{"parameter":"MFR","unit":"kg","values":[{"value":"0,00E+00","module":"A1-A3","scenario":null},{"value":"0,00E+00","module":"C1","scenario":null},{"value":"0,00E+00","module":"C2","scenario":null},{"value":"9,80E+02","module":"C3","scenario":null},{"value":"0,00E+00","module":"C4","scenario":null},{"value":"0,00E+00","module":"D","scenario":null}]},{"parameter":"MER","unit":"kg","values":[{"value":"0,00E+00","module":"A1-A3","scenario":null},{"value":"0,00E+00","module":"C1","scenario":null},{"value":"0,00E+00","module":"C2","scenario":null},{"value":"0,00E+00","module":"C3","scenario":null},{"value":"0,00E+00","module":"C4","scenario":null},{"value":"0,00E+00","module":"D","scenario":null}]},{"parameter":"EEE","unit":"MJ","values":[{"value":"0,00E+00","module":"A1-A3","scenario":null},{"value":"0,00E+00","module":"C1","scenario":null},{"value":"0,00E+00","module":"C2","scenario":null},{"value":"0,00E+00","module":"C3","scenario":null},{"value":"0,00E+00","module":"C4","scenario":null},{"value":"0,00E+00","module":"D","scenario":null}]},{"parameter":"EET","unit":"MJ","values":[{"value":"0,00E+00","module":"A1-A3","scenario":null},{"value":"0,00E+00","module":"C1","scenario":null},{"value":"0,00E+00","module":"C2","scenario":null},{"value":"0,00E+00","module":"C3","scenario":null},{"value":"0,00E+00","module":"C4","scenario":null},{"value":"0,00E+00","module":"D","scenario":null}]}]}