{"product_name":"Reinforcing stabilized three and seven-wire strands with and without dents with a nominal tensile strength of 1670\u00f71860 N /mm2 with a diameter of 6.5\u00f715.7 mm (PC-strand)","epd_id":"EPD-Kiwa-EE-162692-EN","compliance":["EN 15804+A2","ISO 14025"],"producer_name":"PJSC \"STALKANAT\"","environmental_impact":[{"parameter":"GWP-total","unit":"kg CO2-eq.","values":[{"value":"2,54E+00","module":"A1","scenario":"Standard scenario"},{"value":"2,27E-02","module":"A2","scenario":"Standard scenario"},{"value":"2,71E-01","module":"A3","scenario":"Standard scenario"},{"value":"0,00E+00","module":"C1","scenario":"Standard scenario"},{"value":"7,09E-03","module":"C2","scenario":"Standard scenario"},{"value":"0,00E+00","module":"C3","scenario":"Standard scenario"},{"value":"2,64E-04","module":"C4","scenario":"Standard scenario"},{"value":"-1,34E+00","module":"D","scenario":"Standard scenario"},{"value":"2,83E+00","module":"A1A3","scenario":null}]},{"parameter":"GWP-fossil","unit":"kg CO2-eq.","values":[{"value":"2,54E+00","module":"A1","scenario":"Standard scenario"},{"value":"2,25E-02","module":"A2","scenario":"Standard scenario"},{"value":"2,60E-01","module":"A3","scenario":"Standard scenario"},{"value":"0,00E+00","module":"C1","scenario":"Standard scenario"},{"value":"7,09E-03","module":"C2","scenario":"Standard scenario"},{"value":"0,00E+00","module":"C3","scenario":"Standard scenario"},{"value":"2,63E-04","module":"C4","scenario":"Standard scenario"},{"value":"-1,35E+00","module":"D","scenario":"Standard scenario"},{"value":"2,82E+00","module":"A1A3","scenario":null}]},{"parameter":"GWP-biogenic","unit":"kg CO2-eq.","values":[{"value":"-3,12E-03","module":"A1","scenario":"Standard scenario"},{"value":"1,29E-04","module":"A2","scenario":"Standard scenario"},{"value":"2,83E-03","module":"A3","scenario":"Standard scenario"},{"value":"0,00E+00","module":"C1","scenario":"Standard scenario"},{"value":"3,27E-06","module":"C2","scenario":"Standard scenario"},{"value":"0,00E+00","module":"C3","scenario":"Standard scenario"},{"value":"5,22E-07","module":"C4","scenario":"Standard scenario"},{"value":"1,41E-02","module":"D","scenario":"Standard scenario"},{"value":"-1,61E-04","module":"A1A3","scenario":null}]},{"parameter":"GWP-luluc","unit":"kg CO2-eq.","values":[{"value":"3,35E-04","module":"A1","scenario":"Standard scenario"},{"value":"2,67E-05","module":"A2","scenario":"Standard scenario"},{"value":"8,14E-03","module":"A3","scenario":"Standard scenario"},{"value":"0,00E+00","module":"C1","scenario":"Standard scenario"},{"value":"2,60E-06","module":"C2","scenario":"Standard scenario"},{"value":"0,00E+00","module":"C3","scenario":"Standard scenario"},{"value":"7,34E-08","module":"C4","scenario":"Standard scenario"},{"value":"9,99E-04","module":"D","scenario":"Standard scenario"},{"value":"8,50E-03","module":"A1A3","scenario":null}]},{"parameter":"ODP","unit":"kg CFC 11-equiv.","values":[{"value":"2,00E-15","module":"A1","scenario":"Standard scenario"},{"value":"3,08E-09","module":"A2","scenario":"Standard scenario"},{"value":"8,18E-09","module":"A3","scenario":"Standard scenario"},{"value":"0,00E+00","module":"C1","scenario":"Standard scenario"},{"value":"1,56E-09","module":"C2","scenario":"Standard scenario"},{"value":"0,00E+00","module":"C3","scenario":"Standard scenario"},{"value":"1,08E-10","module":"C4","scenario":"Standard scenario"},{"value":"-3,30E-08","module":"D","scenario":"Standard scenario"},{"value":"1,13E-08","module":"A1A3","scenario":null}]},{"parameter":"AP","unit":"mol H+-eq.","values":[{"value":"2,92E-03","module":"A1","scenario":"Standard scenario"},{"value":"1,92E-04","module":"A2","scenario":"Standard scenario"},{"value":"1,01E-03","module":"A3","scenario":"Standard scenario"},{"value":"0,00E+00","module":"C1","scenario":"Standard scenario"},{"value":"4,11E-05","module":"C2","scenario":"Standard scenario"},{"value":"0,00E+00","module":"C3","scenario":"Standard scenario"},{"value":"2,50E-06","module":"C4","scenario":"Standard scenario"},{"value":"-5,22E-03","module":"D","scenario":"Standard scenario"},{"value":"4,12E-03","module":"A1A3","scenario":null}]},{"parameter":"POCP","unit":"kg NMVOC-eq.","values":[{"value":"1,28E-07","module":"A1","scenario":"Standard scenario"},{"value":"2,03E-04","module":"A2","scenario":"Standard scenario"},{"value":"3,35E-04","module":"A3","scenario":"Standard scenario"},{"value":"0,00E+00","module":"C1","scenario":"Standard scenario"},{"value":"4,56E-05","module":"C2","scenario":"Standard scenario"},{"value":"0,00E+00","module":"C3","scenario":"Standard scenario"},{"value":"2,75E-06","module":"C4","scenario":"Standard scenario"},{"value":"-7,69E-03","module":"D","scenario":"Standard scenario"},{"value":"5,38E-04","module":"A1A3","scenario":null}]},{"parameter":"ADPE","unit":"kg Sb-eq.","values":[{"value":"2,60E+01","module":"A1","scenario":"Standard scenario"},{"value":"1,81E-07","module":"A2","scenario":"Standard scenario"},{"value":"6,97E-01","module":"A3","scenario":"Standard scenario"},{"value":"0,00E+00","module":"C1","scenario":"Standard scenario"},{"value":"1,80E-07","module":"C2","scenario":"Standard scenario"},{"value":"0,00E+00","module":"C3","scenario":"Standard scenario"},{"value":"2,41E-09","module":"C4","scenario":"Standard scenario"},{"value":"-9,14E-07","module":"D","scenario":"Standard scenario"},{"value":"2,67E+01","module":"A1A3","scenario":null}]},{"parameter":"ADPF","unit":"MJ","values":[{"value":"5,06E+00","module":"A1","scenario":"Standard scenario"},{"value":"3,31E-01","module":"A2","scenario":"Standard scenario"},{"value":"1,86E+00","module":"A3","scenario":"Standard scenario"},{"value":"0,00E+00","module":"C1","scenario":"Standard scenario"},{"value":"1,07E-01","module":"C2","scenario":"Standard scenario"},{"value":"0,00E+00","module":"C3","scenario":"Standard scenario"},{"value":"7,36E-03","module":"C4","scenario":"Standard scenario"},{"value":"-9,45E+00","module":"D","scenario":"Standard scenario"},{"value":"7,25E+00","module":"A1A3","scenario":null}]},{"parameter":"WDP","unit":"m3 world-eq.","values":[{"value":"2,78E-08","module":"A1","scenario":"Standard scenario"},{"value":"2,92E-03","module":"A2","scenario":"Standard scenario"},{"value":"6,38E-01","module":"A3","scenario":"Standard scenario"},{"value":"0,00E+00","module":"C1","scenario":"Standard scenario"},{"value":"3,82E-04","module":"C2","scenario":"Standard scenario"},{"value":"0,00E+00","module":"C3","scenario":"Standard scenario"},{"value":"3,30E-04","module":"C4","scenario":"Standard scenario"},{"value":"-2,58E-01","module":"D","scenario":"Standard scenario"},{"value":"6,41E-01","module":"A1A3","scenario":null}]},{"parameter":"EP-freshwater","unit":"kg P-eq.","values":[{"value":"3,49E+00","module":"A1","scenario":"Standard scenario"},{"value":"9,51E-07","module":"A2","scenario":"Standard scenario"},{"value":"9,36E-02","module":"A3","scenario":"Standard scenario"},{"value":"0,00E+00","module":"C1","scenario":"Standard scenario"},{"value":"7,15E-08","module":"C2","scenario":"Standard scenario"},{"value":"0,00E+00","module":"C3","scenario":"Standard scenario"},{"value":"2,95E-09","module":"C4","scenario":"Standard scenario"},{"value":"-4,78E-05","module":"D","scenario":"Standard scenario"},{"value":"3,58E+00","module":"A1A3","scenario":null}]},{"parameter":"EP-marine","unit":"kg N-eq.","values":[{"value":"6,15E-03","module":"A1","scenario":"Standard scenario"},{"value":"6,74E-05","module":"A2","scenario":"Standard scenario"},{"value":"3,53E-04","module":"A3","scenario":"Standard scenario"},{"value":"0,00E+00","module":"C1","scenario":"Standard scenario"},{"value":"1,45E-05","module":"C2","scenario":"Standard scenario"},{"value":"0,00E+00","module":"C3","scenario":"Standard scenario"},{"value":"8,60E-07","module":"C4","scenario":"Standard scenario"},{"value":"-9,68E-04","module":"D","scenario":"Standard scenario"},{"value":"6,57E-03","module":"A1A3","scenario":null}]},{"parameter":"EP-terrestrial","unit":"mol N-eq.","values":[{"value":"1,65E-03","module":"A1","scenario":"Standard scenario"},{"value":"7,47E-04","module":"A2","scenario":"Standard scenario"},{"value":"1,62E-03","module":"A3","scenario":"Standard scenario"},{"value":"0,00E+00","module":"C1","scenario":"Standard scenario"},{"value":"1,60E-04","module":"C2","scenario":"Standard scenario"},{"value":"0,00E+00","module":"C3","scenario":"Standard scenario"},{"value":"9,48E-06","module":"C4","scenario":"Standard scenario"},{"value":"-1,13E-02","module":"D","scenario":"Standard scenario"},{"value":"4,02E-03","module":"A1A3","scenario":null}]}],"additional_environmental_impact":[{"parameter":"PM","unit":"disease incidence","values":[{"value":"6,15E-03","module":"A1","scenario":"Standard scenario"},{"value":"1,68E-09","module":"A2","scenario":"Standard scenario"},{"value":"1,65E-04","module":"A3","scenario":"Standard scenario"},{"value":"0,00E+00","module":"C1","scenario":"Standard scenario"},{"value":"6,37E-10","module":"C2","scenario":"Standard scenario"},{"value":"0,00E+00","module":"C3","scenario":"Standard scenario"},{"value":"4,86E-11","module":"C4","scenario":"Standard scenario"},{"value":"-7,83E-08","module":"D","scenario":"Standard scenario"},{"value":"6,32E-03","module":"A1A3","scenario":null}]},{"parameter":"ETP-fw","unit":"CTUe","values":[{"value":"3,49E+00","module":"A1","scenario":"Standard scenario"},{"value":"3,54E-01","module":"A2","scenario":"Standard scenario"},{"value":"3,23E+00","module":"A3","scenario":"Standard scenario"},{"value":"0,00E+00","module":"C1","scenario":"Standard scenario"},{"value":"9,53E-02","module":"C2","scenario":"Standard scenario"},{"value":"0,00E+00","module":"C3","scenario":"Standard scenario"},{"value":"4,77E-03","module":"C4","scenario":"Standard scenario"},{"value":"-4,54E+01","module":"D","scenario":"Standard scenario"},{"value":"7,07E+00","module":"A1A3","scenario":null}]},{"parameter":"HTP-c","unit":"CTUh","values":[{"value":"1,23E-10","module":"A1","scenario":"Standard scenario"},{"value":"2,16E-11","module":"A2","scenario":"Standard scenario"},{"value":"1,03E-09","module":"A3","scenario":"Standard scenario"},{"value":"0,00E+00","module":"C1","scenario":"Standard scenario"},{"value":"3,09E-12","module":"C2","scenario":"Standard scenario"},{"value":"0,00E+00","module":"C3","scenario":"Standard scenario"},{"value":"1,10E-13","module":"C4","scenario":"Standard scenario"},{"value":"-1,75E-10","module":"D","scenario":"Standard scenario"},{"value":"1,17E-09","module":"A1A3","scenario":null}]},{"parameter":"HTP-nc","unit":"CTUh","values":[{"value":"1,12E-08","module":"A1","scenario":"Standard scenario"},{"value":"3,96E-10","module":"A2","scenario":"Standard scenario"},{"value":"1,28E-08","module":"A3","scenario":"Standard scenario"},{"value":"0,00E+00","module":"C1","scenario":"Standard scenario"},{"value":"1,04E-10","module":"C2","scenario":"Standard scenario"},{"value":"0,00E+00","module":"C3","scenario":"Standard scenario"},{"value":"3,39E-12","module":"C4","scenario":"Standard scenario"},{"value":"2,62E-07","module":"D","scenario":"Standard scenario"},{"value":"2,44E-08","module":"A1A3","scenario":null}]},{"parameter":"SQP","unit":"dimensionless","values":[{"value":"1,64E+00","module":"A1","scenario":"Standard scenario"},{"value":"2,28E-01","module":"A2","scenario":"Standard scenario"},{"value":"8,33E-01","module":"A3","scenario":"Standard scenario"},{"value":"0,00E+00","module":"C1","scenario":"Standard scenario"},{"value":"9,27E-02","module":"C2","scenario":"Standard scenario"},{"value":"0,00E+00","module":"C3","scenario":"Standard scenario"},{"value":"1,54E-02","module":"C4","scenario":"Standard scenario"},{"value":"-2,09E+00","module":"D","scenario":"Standard scenario"},{"value":"2,70E+00","module":"A1A3","scenario":null}]},{"parameter":"IRP","unit":"kBq U235-eq.","values":[{"value":"5,22E-02","module":"A1","scenario":"Standard scenario"},{"value":"1,85E-03","module":"A2","scenario":"Standard scenario"},{"value":"1,62E-02","module":"A3","scenario":"Standard scenario"},{"value":"0,00E+00","module":"C1","scenario":"Standard scenario"},{"value":"4,48E-04","module":"C2","scenario":"Standard scenario"},{"value":"0,00E+00","module":"C3","scenario":"Standard scenario"},{"value":"3,02E-05","module":"C4","scenario":"Standard scenario"},{"value":"2,31E-02","module":"D","scenario":"Standard scenario"},{"value":"7,03E-02","module":"A1A3","scenario":null}]}],"resource_use":[{"parameter":"PERE","unit":"MJ","values":[{"value":"4,94E-01","module":"A1","scenario":"Standard scenario"},{"value":"2,85E-02","module":"A2","scenario":"Standard scenario"},{"value":"1,63E-01","module":"A3","scenario":"Standard scenario"},{"value":"0,00E+00","module":"C1","scenario":"Standard scenario"},{"value":"1,34E-03","module":"C2","scenario":"Standard scenario"},{"value":"0,00E+00","module":"C3","scenario":"Standard scenario"},{"value":"5,95E-05","module":"C4","scenario":"Standard scenario"},{"value":"2,75E-01","module":"D","scenario":"Standard scenario"},{"value":"6,85E-01","module":"A1A3","scenario":null}]},{"parameter":"PERM","unit":"MJ","values":[{"value":"0,00E+00","module":"A1","scenario":"Standard scenario"},{"value":"0,00E+00","module":"A2","scenario":"Standard scenario"},{"value":"0,00E+00","module":"A3","scenario":"Standard scenario"},{"value":"0,00E+00","module":"C1","scenario":"Standard scenario"},{"value":"0,00E+00","module":"C2","scenario":"Standard scenario"},{"value":"0,00E+00","module":"C3","scenario":"Standard scenario"},{"value":"0,00E+00","module":"C4","scenario":"Standard scenario"},{"value":"0,00E+00","module":"D","scenario":"Standard scenario"},{"value":"0,00E+00","module":"A1A3","scenario":null}]},{"parameter":"PERT","unit":"MJ","values":[{"value":"4,94E-01","module":"A1","scenario":"Standard scenario"},{"value":"2,85E-02","module":"A2","scenario":"Standard scenario"},{"value":"1,63E-01","module":"A3","scenario":"Standard scenario"},{"value":"0,00E+00","module":"C1","scenario":"Standard scenario"},{"value":"1,34E-03","module":"C2","scenario":"Standard scenario"},{"value":"0,00E+00","module":"C3","scenario":"Standard scenario"},{"value":"5,95E-05","module":"C4","scenario":"Standard scenario"},{"value":"2,75E-01","module":"D","scenario":"Standard scenario"},{"value":"6,85E-01","module":"A1A3","scenario":null}]},{"parameter":"PENRE","unit":"MJ","values":[{"value":"2,60E+01","module":"A1","scenario":"Standard scenario"},{"value":"3,50E-01","module":"A2","scenario":"Standard scenario"},{"value":"2,44E+00","module":"A3","scenario":"Standard scenario"},{"value":"0,00E+00","module":"C1","scenario":"Standard scenario"},{"value":"1,13E-01","module":"C2","scenario":"Standard scenario"},{"value":"0,00E+00","module":"C3","scenario":"Standard scenario"},{"value":"7,82E-03","module":"C4","scenario":"Standard scenario"},{"value":"-9,81E+00","module":"D","scenario":"Standard scenario"},{"value":"2,88E+01","module":"A1A3","scenario":null}]},{"parameter":"PENRM","unit":"MJ","values":[{"value":"0,00E+00","module":"A1","scenario":"Standard scenario"},{"value":"0,00E+00","module":"A2","scenario":"Standard scenario"},{"value":"5,66E-02","module":"A3","scenario":"Standard scenario"},{"value":"0,00E+00","module":"C1","scenario":"Standard scenario"},{"value":"0,00E+00","module":"C2","scenario":"Standard scenario"},{"value":"0,00E+00","module":"C3","scenario":"Standard scenario"},{"value":"0,00E+00","module":"C4","scenario":"Standard scenario"},{"value":"0,00E+00","module":"D","scenario":"Standard scenario"},{"value":"5,66E-02","module":"A1A3","scenario":null}]},{"parameter":"PENRT","unit":"MJ","values":[{"value":"2,60E+01","module":"A1","scenario":"Standard scenario"},{"value":"3,50E-01","module":"A2","scenario":"Standard scenario"},{"value":"2,50E+00","module":"A3","scenario":"Standard scenario"},{"value":"0,00E+00","module":"C1","scenario":"Standard scenario"},{"value":"1,13E-01","module":"C2","scenario":"Standard scenario"},{"value":"0,00E+00","module":"C3","scenario":"Standard scenario"},{"value":"7,82E-03","module":"C4","scenario":"Standard scenario"},{"value":"-9,81E+00","module":"D","scenario":"Standard scenario"},{"value":"2,89E+01","module":"A1A3","scenario":null}]},{"parameter":"SM","unit":"kg","values":[{"value":"1,67E-01","module":"A1","scenario":"Standard scenario"},{"value":"0,00E+00","module":"A2","scenario":"Standard scenario"},{"value":"5,16E-03","module":"A3","scenario":"Standard scenario"},{"value":"0,00E+00","module":"C1","scenario":"Standard scenario"},{"value":"0,00E+00","module":"C2","scenario":"Standard scenario"},{"value":"0,00E+00","module":"C3","scenario":"Standard scenario"},{"value":"0,00E+00","module":"C4","scenario":"Standard scenario"},{"value":"0,00E+00","module":"D","scenario":"Standard scenario"},{"value":"1,72E-01","module":"A1A3","scenario":null}]},{"parameter":"RSF","unit":"MJ","values":[{"value":"0,00E+00","module":"A1","scenario":"Standard scenario"},{"value":"0,00E+00","module":"A2","scenario":"Standard scenario"},{"value":"0,00E+00","module":"A3","scenario":"Standard scenario"},{"value":"0,00E+00","module":"C1","scenario":"Standard scenario"},{"value":"0,00E+00","module":"C2","scenario":"Standard scenario"},{"value":"0,00E+00","module":"C3","scenario":"Standard scenario"},{"value":"0,00E+00","module":"C4","scenario":"Standard scenario"},{"value":"0,00E+00","module":"D","scenario":"Standard scenario"},{"value":"0,00E+00","module":"A1A3","scenario":null}]},{"parameter":"NRSF","unit":"MJ","values":[{"value":"0,00E+00","module":"A1","scenario":"Standard scenario"},{"value":"0,00E+00","module":"A2","scenario":"Standard scenario"},{"value":"0,00E+00","module":"A3","scenario":"Standard scenario"},{"value":"0,00E+00","module":"C1","scenario":"Standard scenario"},{"value":"0,00E+00","module":"C2","scenario":"Standard scenario"},{"value":"0,00E+00","module":"C3","scenario":"Standard scenario"},{"value":"0,00E+00","module":"C4","scenario":"Standard scenario"},{"value":"0,00E+00","module":"D","scenario":"Standard scenario"},{"value":"0,00E+00","module":"A1A3","scenario":null}]},{"parameter":"FW","unit":"m3","values":[{"value":"1,19E-01","module":"A1","scenario":"Standard scenario"},{"value":"1,55E-04","module":"A2","scenario":"Standard scenario"},{"value":"1,84E-02","module":"A3","scenario":"Standard scenario"},{"value":"0,00E+00","module":"C1","scenario":"Standard scenario"},{"value":"1,30E-05","module":"C2","scenario":"Standard scenario"},{"value":"0,00E+00","module":"C3","scenario":"Standard scenario"},{"value":"7,86E-06","module":"C4","scenario":"Standard scenario"},{"value":"-4,89E-03","module":"D","scenario":"Standard scenario"},{"value":"1,38E-01","module":"A1A3","scenario":null}]}],"end_of_life_waste":[{"parameter":"HWD","unit":"kg","values":[{"value":"1,92E-09","module":"A1","scenario":"Standard scenario"},{"value":"6,42E-07","module":"A2","scenario":"Standard scenario"},{"value":"4,27E-06","module":"A3","scenario":"Standard scenario"},{"value":"0,00E+00","module":"C1","scenario":"Standard scenario"},{"value":"2,71E-07","module":"C2","scenario":"Standard scenario"},{"value":"0,00E+00","module":"C3","scenario":"Standard scenario"},{"value":"1,10E-08","module":"C4","scenario":"Standard scenario"},{"value":"-1,62E-04","module":"D","scenario":"Standard scenario"},{"value":"4,91E-06","module":"A1A3","scenario":null}]},{"parameter":"NHWD","unit":"kg","values":[{"value":"2,36E-01","module":"A1","scenario":"Standard scenario"},{"value":"4,46E-03","module":"A2","scenario":"Standard scenario"},{"value":"1,01E-01","module":"A3","scenario":"Standard scenario"},{"value":"0,00E+00","module":"C1","scenario":"Standard scenario"},{"value":"6,78E-03","module":"C2","scenario":"Standard scenario"},{"value":"0,00E+00","module":"C3","scenario":"Standard scenario"},{"value":"5,00E-02","module":"C4","scenario":"Standard scenario"},{"value":"-1,32E-01","module":"D","scenario":"Standard scenario"},{"value":"3,41E-01","module":"A1A3","scenario":null}]},{"parameter":"RWD","unit":"kg","values":[{"value":"6,56E-04","module":"A1","scenario":"Standard scenario"},{"value":"2,03E-06","module":"A2","scenario":"Standard scenario"},{"value":"3,01E-05","module":"A3","scenario":"Standard scenario"},{"value":"0,00E+00","module":"C1","scenario":"Standard scenario"},{"value":"7,02E-07","module":"C2","scenario":"Standard scenario"},{"value":"0,00E+00","module":"C3","scenario":"Standard scenario"},{"value":"4,83E-08","module":"C4","scenario":"Standard scenario"},{"value":"8,01E-06","module":"D","scenario":"Standard scenario"},{"value":"6,88E-04","module":"A1A3","scenario":null}]}],"end_of_life_flow":[{"parameter":"CRU","unit":"kg","values":[{"value":"0,00E+00","module":"A1","scenario":"Standard scenario"},{"value":"0,00E+00","module":"A2","scenario":"Standard scenario"},{"value":"0,00E+00","module":"A3","scenario":"Standard scenario"},{"value":"0,00E+00","module":"C1","scenario":"Standard scenario"},{"value":"0,00E+00","module":"C2","scenario":"Standard scenario"},{"value":"0,00E+00","module":"C3","scenario":"Standard scenario"},{"value":"0,00E+00","module":"C4","scenario":"Standard scenario"},{"value":"0,00E+00","module":"D","scenario":"Standard scenario"},{"value":"0,00E+00","module":"A1A3","scenario":null}]},{"parameter":"MFR","unit":"kg","values":[{"value":"4,52E-04","module":"A1","scenario":"Standard scenario"},{"value":"0,00E+00","module":"A2","scenario":"Standard scenario"},{"value":"2,55E-02","module":"A3","scenario":"Standard scenario"},{"value":"0,00E+00","module":"C1","scenario":"Standard scenario"},{"value":"0,00E+00","module":"C2","scenario":"Standard scenario"},{"value":"9,50E-01","module":"C3","scenario":"Standard scenario"},{"value":"0,00E+00","module":"C4","scenario":"Standard scenario"},{"value":"0,00E+00","module":"D","scenario":"Standard scenario"},{"value":"2,60E-02","module":"A1A3","scenario":null}]},{"parameter":"MER","unit":"kg","values":[{"value":"0,00E+00","module":"A1","scenario":"Standard scenario"},{"value":"0,00E+00","module":"A2","scenario":"Standard scenario"},{"value":"0,00E+00","module":"A3","scenario":"Standard scenario"},{"value":"0,00E+00","module":"C1","scenario":"Standard scenario"},{"value":"0,00E+00","module":"C2","scenario":"Standard scenario"},{"value":"0,00E+00","module":"C3","scenario":"Standard scenario"},{"value":"0,00E+00","module":"C4","scenario":"Standard scenario"},{"value":"0,00E+00","module":"D","scenario":"Standard scenario"},{"value":"0,00E+00","module":"A1A3","scenario":null}]},{"parameter":"EEE","unit":"MJ","values":[{"value":"0,00E+00","module":"A1","scenario":"Standard scenario"},{"value":"0,00E+00","module":"A2","scenario":"Standard scenario"},{"value":"8,12E-03","module":"A3","scenario":"Standard scenario"},{"value":"0,00E+00","module":"C1","scenario":"Standard scenario"},{"value":"0,00E+00","module":"C2","scenario":"Standard scenario"},{"value":"0,00E+00","module":"C3","scenario":"Standard scenario"},{"value":"0,00E+00","module":"C4","scenario":"Standard scenario"},{"value":"0,00E+00","module":"D","scenario":"Standard scenario"},{"value":"8,12E-03","module":"A1A3","scenario":null}]},{"parameter":"EET","unit":"MJ","values":[{"value":"0,00E+00","module":"A1","scenario":"Standard scenario"},{"value":"0,00E+00","module":"A2","scenario":"Standard scenario"},{"value":"1,40E-02","module":"A3","scenario":"Standard scenario"},{"value":"0,00E+00","module":"C1","scenario":"Standard scenario"},{"value":"0,00E+00","module":"C2","scenario":"Standard scenario"},{"value":"0,00E+00","module":"C3","scenario":"Standard scenario"},{"value":"0,00E+00","module":"C4","scenario":"Standard scenario"},{"value":"0,00E+00","module":"D","scenario":"Standard scenario"},{"value":"1,40E-02","module":"A1A3","scenario":null}]}]}