{"product_name":"GTBUILD - Galvanized coated steel sheet metal - Published in according to MRA agreement with EPD China","epd_id":"EPD-CN-00011","compliance":["EN 15804+A2","ISO 14025","ISO 21930"],"producer_name":"Taicang Gronsedt Technology Co., Ltd.","environmental_impact":[{"parameter":"GWP-total","unit":"kg CO2-eq.","values":[{"value":"5,18E+00","module":"A1-A3","scenario":null},{"value":"2,25E-01","module":"A4","scenario":null},{"value":"9,30E-03","module":"A5","scenario":null},{"value":"0,00E+00","module":"C1","scenario":null},{"value":"1,56E-02","module":"C2","scenario":null},{"value":"5,50E-02","module":"C3","scenario":null},{"value":"0,00E+00","module":"C4","scenario":null},{"value":"-1,84E+00","module":"D","scenario":null}]},{"parameter":"GWP-fossil","unit":"kg CO2-eq.","values":[{"value":"5,14E+00","module":"A1-A3","scenario":null},{"value":"2,25E-01","module":"A4","scenario":null},{"value":"7,61E-03","module":"A5","scenario":null},{"value":"0,00E+00","module":"C1","scenario":null},{"value":"1,56E-02","module":"C2","scenario":null},{"value":"4,58E-02","module":"C3","scenario":null},{"value":"0,00E+00","module":"C4","scenario":null},{"value":"-1,85E+00","module":"D","scenario":null}]},{"parameter":"GWP-biogenic","unit":"kg CO2-eq.","values":[{"value":"1,58E-01","module":"A1-A3","scenario":null},{"value":"-6,44E-05","module":"A4","scenario":null},{"value":"-1,21E-01","module":"A5","scenario":null},{"value":"0,00E+00","module":"C1","scenario":null},{"value":"9,19E-07","module":"C2","scenario":null},{"value":"9,06E-03","module":"C3","scenario":null},{"value":"0,00E+00","module":"C4","scenario":null},{"value":"8,94E-03","module":"D","scenario":null}]},{"parameter":"GWP-luluc","unit":"kg CO2-eq.","values":[{"value":"3,40E-03","module":"A1-A3","scenario":null},{"value":"1,16E-04","module":"A4","scenario":null},{"value":"6,92E-06","module":"A5","scenario":null},{"value":"0,00E+00","module":"C1","scenario":null},{"value":"6,37E-06","module":"C2","scenario":null},{"value":"9,23E-05","module":"C3","scenario":null},{"value":"0,00E+00","module":"C4","scenario":null},{"value":"-3,03E-04","module":"D","scenario":null}]},{"parameter":"ODP","unit":"kg CFC 11-eq.","values":[{"value":"4,28E-08","module":"A1-A3","scenario":null},{"value":"3,23E-09","module":"A4","scenario":null},{"value":"7,10E-11","module":"A5","scenario":null},{"value":"0,00E+00","module":"C1","scenario":null},{"value":"2,27E-10","module":"C2","scenario":null},{"value":"7,31E-10","module":"C3","scenario":null},{"value":"0,00E+00","module":"C4","scenario":null},{"value":"-4,61E-09","module":"D","scenario":null}]},{"parameter":"AP","unit":"mol H+-eq.","values":[{"value":"2,16E-02","module":"A1-A3","scenario":null},{"value":"6,16E-03","module":"A4","scenario":null},{"value":"3,25E-05","module":"A5","scenario":null},{"value":"0,00E+00","module":"C1","scenario":null},{"value":"7,09E-05","module":"C2","scenario":null},{"value":"2,27E-04","module":"C3","scenario":null},{"value":"0,00E+00","module":"C4","scenario":null},{"value":"-6,05E-03","module":"D","scenario":null}]},{"parameter":"POCP","unit":"kg NMVOC-eq.","values":[{"value":"1,61E-02","module":"A1-A3","scenario":null},{"value":"4,66E-03","module":"A4","scenario":null},{"value":"4,36E-05","module":"A5","scenario":null},{"value":"0,00E+00","module":"C1","scenario":null},{"value":"1,00E-04","module":"C2","scenario":null},{"value":"2,96E-04","module":"C3","scenario":null},{"value":"0,00E+00","module":"C4","scenario":null},{"value":"-5,02E-03","module":"D","scenario":null}]},{"parameter":"ADPE","unit":"kg Sb-eq.","values":[{"value":"3,84E-05","module":"A1-A3","scenario":null},{"value":"2,55E-07","module":"A4","scenario":null},{"value":"1,93E-08","module":"A5","scenario":null},{"value":"0,00E+00","module":"C1","scenario":null},{"value":"4,88E-08","module":"C2","scenario":null},{"value":"1,35E-07","module":"C3","scenario":null},{"value":"0,00E+00","module":"C4","scenario":null},{"value":"-8,51E-07","module":"D","scenario":null}]},{"parameter":"ADPF","unit":"MJ","values":[{"value":"5,68E+01","module":"A1-A3","scenario":null},{"value":"2,79E+00","module":"A4","scenario":null},{"value":"7,08E-02","module":"A5","scenario":null},{"value":"0,00E+00","module":"C1","scenario":null},{"value":"2,22E-01","module":"C2","scenario":null},{"value":"6,36E-01","module":"C3","scenario":null},{"value":"0,00E+00","module":"C4","scenario":null},{"value":"-1,74E+01","module":"D","scenario":null}]},{"parameter":"WDP","unit":"m3 world-eq.","values":[{"value":"9,22E-01","module":"A1-A3","scenario":null},{"value":"7,05E-03","module":"A4","scenario":null},{"value":"4,41E-04","module":"A5","scenario":null},{"value":"0,00E+00","module":"C1","scenario":null},{"value":"1,06E-03","module":"C2","scenario":null},{"value":"2,16E-02","module":"C3","scenario":null},{"value":"0,00E+00","module":"C4","scenario":null},{"value":"-1,21E-01","module":"D","scenario":null}]},{"parameter":"EP-freshwater","unit":"kg P-eq.","values":[{"value":"1,80E-03","module":"A1-A3","scenario":null},{"value":"7,98E-06","module":"A4","scenario":null},{"value":"7,68E-07","module":"A5","scenario":null},{"value":"0,00E+00","module":"C1","scenario":null},{"value":"1,25E-06","module":"C2","scenario":null},{"value":"3,11E-05","module":"C3","scenario":null},{"value":"0,00E+00","module":"C4","scenario":null},{"value":"-4,73E-04","module":"D","scenario":null}]},{"parameter":"EP-marine","unit":"kg N-eq.","values":[{"value":"4,80E-03","module":"A1-A3","scenario":null},{"value":"1,54E-03","module":"A4","scenario":null},{"value":"1,30E-05","module":"A5","scenario":null},{"value":"0,00E+00","module":"C1","scenario":null},{"value":"2,66E-05","module":"C2","scenario":null},{"value":"8,13E-05","module":"C3","scenario":null},{"value":"0,00E+00","module":"C4","scenario":null},{"value":"-1,36E-03","module":"D","scenario":null}]},{"parameter":"EP-terrestrial","unit":"mol N-eq.","values":[{"value":"4,91E-02","module":"A1-A3","scenario":null},{"value":"1,71E-02","module":"A4","scenario":null},{"value":"1,24E-04","module":"A5","scenario":null},{"value":"0,00E+00","module":"C1","scenario":null},{"value":"2,90E-04","module":"C2","scenario":null},{"value":"8,77E-04","module":"C3","scenario":null},{"value":"0,00E+00","module":"C4","scenario":null},{"value":"-1,48E-02","module":"D","scenario":null}]},{"parameter":"GWP-IOBC","unit":"kg CO2-eq.","values":[]}],"additional_environmental_impact":[{"parameter":"PM","unit":"disease incidence","values":[{"value":"0,00E+00","module":"A1-A3","scenario":null},{"value":"0,00E+00","module":"A4","scenario":null},{"value":"0,00E+00","module":"A5","scenario":null},{"value":"0,00E+00","module":"C1","scenario":null},{"value":"0,00E+00","module":"C2","scenario":null},{"value":"0,00E+00","module":"C3","scenario":null},{"value":"0,00E+00","module":"C4","scenario":null},{"value":"0,00E+00","module":"D","scenario":null}]},{"parameter":"ETP-fw","unit":"CTUe","values":[{"value":"0,00E+00","module":"A1-A3","scenario":null},{"value":"0,00E+00","module":"A4","scenario":null},{"value":"0,00E+00","module":"A5","scenario":null},{"value":"0,00E+00","module":"C1","scenario":null},{"value":"0,00E+00","module":"C2","scenario":null},{"value":"0,00E+00","module":"C3","scenario":null},{"value":"0,00E+00","module":"C4","scenario":null},{"value":"0,00E+00","module":"D","scenario":null}]},{"parameter":"HTP-c","unit":"CTUh","values":[{"value":"0,00E+00","module":"A1-A3","scenario":null},{"value":"0,00E+00","module":"A4","scenario":null},{"value":"0,00E+00","module":"A5","scenario":null},{"value":"0,00E+00","module":"C1","scenario":null},{"value":"0,00E+00","module":"C2","scenario":null},{"value":"0,00E+00","module":"C3","scenario":null},{"value":"0,00E+00","module":"C4","scenario":null},{"value":"0,00E+00","module":"D","scenario":null}]},{"parameter":"HTP-nc","unit":"CTUh","values":[{"value":"0,00E+00","module":"A1-A3","scenario":null},{"value":"0,00E+00","module":"A4","scenario":null},{"value":"0,00E+00","module":"A5","scenario":null},{"value":"0,00E+00","module":"C1","scenario":null},{"value":"0,00E+00","module":"C2","scenario":null},{"value":"0,00E+00","module":"C3","scenario":null},{"value":"0,00E+00","module":"C4","scenario":null},{"value":"0,00E+00","module":"D","scenario":null}]},{"parameter":"SQP","unit":"unitless","values":[{"value":"0,00E+00","module":"A1-A3","scenario":null},{"value":"0,00E+00","module":"A4","scenario":null},{"value":"0,00E+00","module":"A5","scenario":null},{"value":"0,00E+00","module":"C1","scenario":null},{"value":"0,00E+00","module":"C2","scenario":null},{"value":"0,00E+00","module":"C3","scenario":null},{"value":"0,00E+00","module":"C4","scenario":null},{"value":"0,00E+00","module":"D","scenario":null}]},{"parameter":"IRP","unit":"kBq U235-eq.","values":[{"value":"0,00E+00","module":"A1-A3","scenario":null},{"value":"0,00E+00","module":"A4","scenario":null},{"value":"0,00E+00","module":"A5","scenario":null},{"value":"0,00E+00","module":"C1","scenario":null},{"value":"0,00E+00","module":"C2","scenario":null},{"value":"0,00E+00","module":"C3","scenario":null},{"value":"0,00E+00","module":"C4","scenario":null},{"value":"0,00E+00","module":"D","scenario":null}]}],"resource_use":[{"parameter":"PERE","unit":"MJ","values":[{"value":"-4,22E+00","module":"A1-A3","scenario":null},{"value":"2,14E-02","module":"A4","scenario":null},{"value":"2,15E-03","module":"A5","scenario":null},{"value":"0,00E+00","module":"C1","scenario":null},{"value":"2,91E-03","module":"C2","scenario":null},{"value":"1,26E-02","module":"C3","scenario":null},{"value":"0,00E+00","module":"C4","scenario":null},{"value":"-3,40E-01","module":"D","scenario":null}]},{"parameter":"PERM","unit":"MJ","values":[{"value":"1,13E+01","module":"A1-A3","scenario":null},{"value":"0,00E+00","module":"A4","scenario":null},{"value":"0,00E+00","module":"A5","scenario":null},{"value":"0,00E+00","module":"C1","scenario":null},{"value":"0,00E+00","module":"C2","scenario":null},{"value":"0,00E+00","module":"C3","scenario":null},{"value":"0,00E+00","module":"C4","scenario":null},{"value":"0,00E+00","module":"D","scenario":null}]},{"parameter":"PERT","unit":"MJ","values":[{"value":"7,10E+00","module":"A1-A3","scenario":null},{"value":"2,14E-02","module":"A4","scenario":null},{"value":"2,15E-03","module":"A5","scenario":null},{"value":"0,00E+00","module":"C1","scenario":null},{"value":"2,91E-03","module":"C2","scenario":null},{"value":"1,26E-02","module":"C3","scenario":null},{"value":"0,00E+00","module":"C4","scenario":null},{"value":"-3,40E-01","module":"D","scenario":null}]},{"parameter":"PENRE","unit":"MJ","values":[{"value":"5,67E+01","module":"A1-A3","scenario":null},{"value":"2,79E+00","module":"A4","scenario":null},{"value":"7,08E-02","module":"A5","scenario":null},{"value":"0,00E+00","module":"C1","scenario":null},{"value":"2,22E-01","module":"C2","scenario":null},{"value":"6,36E-01","module":"C3","scenario":null},{"value":"0,00E+00","module":"C4","scenario":null},{"value":"-1,74E+01","module":"D","scenario":null}]},{"parameter":"PENRM","unit":"MJ","values":[{"value":"9,56E-02","module":"A1-A3","scenario":null},{"value":"0,00E+00","module":"A4","scenario":null},{"value":"0,00E+00","module":"A5","scenario":null},{"value":"0,00E+00","module":"C1","scenario":null},{"value":"0,00E+00","module":"C2","scenario":null},{"value":"0,00E+00","module":"C3","scenario":null},{"value":"0,00E+00","module":"C4","scenario":null},{"value":"0,00E+00","module":"D","scenario":null}]},{"parameter":"PENRT","unit":"MJ","values":[{"value":"5,68E+01","module":"A1-A3","scenario":null},{"value":"2,79E+00","module":"A4","scenario":null},{"value":"7,08E-02","module":"A5","scenario":null},{"value":"0,00E+00","module":"C1","scenario":null},{"value":"2,22E-01","module":"C2","scenario":null},{"value":"6,36E-01","module":"C3","scenario":null},{"value":"0,00E+00","module":"C4","scenario":null},{"value":"-1,74E+01","module":"D","scenario":null}]},{"parameter":"SM","unit":"kg","values":[{"value":"0,00E+00","module":"A1-A3","scenario":null},{"value":"0,00E+00","module":"A4","scenario":null},{"value":"0,00E+00","module":"A5","scenario":null},{"value":"0,00E+00","module":"C1","scenario":null},{"value":"0,00E+00","module":"C2","scenario":null},{"value":"0,00E+00","module":"C3","scenario":null},{"value":"0,00E+00","module":"C4","scenario":null},{"value":"0,00E+00","module":"D","scenario":null}]},{"parameter":"RSF","unit":"MJ","values":[{"value":"0,00E+00","module":"A1-A3","scenario":null},{"value":"0,00E+00","module":"A4","scenario":null},{"value":"0,00E+00","module":"A5","scenario":null},{"value":"0,00E+00","module":"C1","scenario":null},{"value":"0,00E+00","module":"C2","scenario":null},{"value":"0,00E+00","module":"C3","scenario":null},{"value":"0,00E+00","module":"C4","scenario":null},{"value":"0,00E+00","module":"D","scenario":null}]},{"parameter":"NRSF","unit":"MJ","values":[{"value":"0,00E+00","module":"A1-A3","scenario":null},{"value":"0,00E+00","module":"A4","scenario":null},{"value":"0,00E+00","module":"A5","scenario":null},{"value":"0,00E+00","module":"C1","scenario":null},{"value":"0,00E+00","module":"C2","scenario":null},{"value":"0,00E+00","module":"C3","scenario":null},{"value":"0,00E+00","module":"C4","scenario":null},{"value":"0,00E+00","module":"D","scenario":null}]},{"parameter":"FW","unit":"m3","values":[{"value":"3,01E-02","module":"A1-A3","scenario":null},{"value":"2,22E-04","module":"A4","scenario":null},{"value":"1,37E-05","module":"A5","scenario":null},{"value":"0,00E+00","module":"C1","scenario":null},{"value":"3,14E-05","module":"C2","scenario":null},{"value":"6,00E-04","module":"C3","scenario":null},{"value":"0,00E+00","module":"C4","scenario":null},{"value":"-3,22E-03","module":"D","scenario":null}]}],"end_of_life_waste":[{"parameter":"HWD","unit":"kg","values":[{"value":"1,03E-02","module":"A1-A3","scenario":null},{"value":"4,17E-05","module":"A4","scenario":null},{"value":"1,62E-05","module":"A5","scenario":null},{"value":"0,00E+00","module":"C1","scenario":null},{"value":"5,88E-06","module":"C2","scenario":null},{"value":"9,74E-01","module":"C3","scenario":null},{"value":"0,00E+00","module":"C4","scenario":null},{"value":"-3,11E-04","module":"D","scenario":null}]},{"parameter":"NHWD","unit":"kg","values":[{"value":"3,32E-01","module":"A1-A3","scenario":null},{"value":"2,01E-02","module":"A4","scenario":null},{"value":"2,19E-03","module":"A5","scenario":null},{"value":"0,00E+00","module":"C1","scenario":null},{"value":"1,36E-02","module":"C2","scenario":null},{"value":"5,34E-02","module":"C3","scenario":null},{"value":"0,00E+00","module":"C4","scenario":null},{"value":"-3,91E-02","module":"D","scenario":null}]},{"parameter":"RWD","unit":"kg","values":[{"value":"7,27E-05","module":"A1-A3","scenario":null},{"value":"3,34E-07","module":"A4","scenario":null},{"value":"3,28E-08","module":"A5","scenario":null},{"value":"0,00E+00","module":"C1","scenario":null},{"value":"4,71E-08","module":"C2","scenario":null},{"value":"1,74E-07","module":"C3","scenario":null},{"value":"0,00E+00","module":"C4","scenario":null},{"value":"-3,13E-06","module":"D","scenario":null}]}],"end_of_life_flow":[{"parameter":"CRU","unit":"kg","values":[{"value":"0,00E+00","module":"A1-A3","scenario":null},{"value":"0,00E+00","module":"A4","scenario":null},{"value":"0,00E+00","module":"A5","scenario":null},{"value":"0,00E+00","module":"C1","scenario":null},{"value":"0,00E+00","module":"C2","scenario":null},{"value":"0,00E+00","module":"C3","scenario":null},{"value":"0,00E+00","module":"C4","scenario":null},{"value":"0,00E+00","module":"D","scenario":null}]},{"parameter":"MFR","unit":"kg","values":[{"value":"6,87E-02","module":"A1-A3","scenario":null},{"value":"0,00E+00","module":"A4","scenario":null},{"value":"8,16E-02","module":"A5","scenario":null},{"value":"0,00E+00","module":"C1","scenario":null},{"value":"0,00E+00","module":"C2","scenario":null},{"value":"0,00E+00","module":"C3","scenario":null},{"value":"1,00E+00","module":"C4","scenario":null},{"value":"0,00E+00","module":"D","scenario":null}]},{"parameter":"MER","unit":"kg","values":[{"value":"0,00E+00","module":"A1-A3","scenario":null},{"value":"0,00E+00","module":"A4","scenario":null},{"value":"0,00E+00","module":"A5","scenario":null},{"value":"0,00E+00","module":"C1","scenario":null},{"value":"0,00E+00","module":"C2","scenario":null},{"value":"0,00E+00","module":"C3","scenario":null},{"value":"0,00E+00","module":"C4","scenario":null},{"value":"0,00E+00","module":"D","scenario":null}]},{"parameter":"EEE","unit":"MJ","values":[{"value":"0,00E+00","module":"A1-A3","scenario":null},{"value":"0,00E+00","module":"A4","scenario":null},{"value":"0,00E+00","module":"A5","scenario":null},{"value":"0,00E+00","module":"C1","scenario":null},{"value":"0,00E+00","module":"C2","scenario":null},{"value":"0,00E+00","module":"C3","scenario":null},{"value":"0,00E+00","module":"C4","scenario":null},{"value":"0,00E+00","module":"D","scenario":null}]},{"parameter":"EET","unit":"MJ","values":[{"value":"0,00E+00","module":"A1-A3","scenario":null},{"value":"0,00E+00","module":"A4","scenario":null},{"value":"0,00E+00","module":"A5","scenario":null},{"value":"0,00E+00","module":"C1","scenario":null},{"value":"0,00E+00","module":"C2","scenario":null},{"value":"0,00E+00","module":"C3","scenario":null},{"value":"0,00E+00","module":"C4","scenario":null},{"value":"0,00E+00","module":"D","scenario":null}]}]}