{"product_name":"Tufted modular carpet tiles with CQuest Bio backing and a pile material of PA 6 with 100% recycled content","epd_id":"EPD-INT-20200181-CCC1-EN","compliance":["DIN EN 15804","ISO 14025"],"producer_name":"Interface Europe Manufacturing BV","environmental_impact":[{"parameter":"GWP-total","unit":"kg CO2-eq.","values":[{"value":"5,46E+00","module":"A1-A3","scenario":null},{"value":"3,19E-01","module":"A4","scenario":null},{"value":"6,00E-01","module":"A5","scenario":null},{"value":"0,00E+00","module":"B1","scenario":null},{"value":"2,92E-01","module":"B2","scenario":null},{"value":"1,78E-02","module":"C2","scenario":null},{"value":"7,08E+00","module":"C3","scenario":"S2"},{"value":"7,16E+00","module":"C3","scenario":"S3"},{"value":"1,26E+00","module":"C4","scenario":null},{"value":"-1,74E-02","module":"D","scenario":"S0"},{"value":"0,00E+00","module":"D","scenario":"S1"},{"value":"-2,52E-01","module":"D","scenario":"S2"},{"value":"-2,51E-01","module":"D","scenario":"S3"}]},{"parameter":"ODP","unit":"kg CFC11-eq.","values":[{"value":"4,45E-08","module":"A1-A3","scenario":null},{"value":"5,24E-17","module":"A4","scenario":null},{"value":"1,34E-09","module":"A5","scenario":null},{"value":"0,00E+00","module":"B1","scenario":null},{"value":"1,21E-08","module":"B2","scenario":null},{"value":"2,92E-18","module":"C2","scenario":null},{"value":"2,47E-15","module":"C3","scenario":"S2"},{"value":"3,36E-15","module":"C3","scenario":"S3"},{"value":"1,18E-15","module":"C4","scenario":null},{"value":"-2,44E-16","module":"D","scenario":"S0"},{"value":"0,00E+00","module":"D","scenario":"S1"},{"value":"-3,46E-15","module":"D","scenario":"S2"},{"value":"-1,47E-15","module":"D","scenario":"S3"}]},{"parameter":"AP","unit":"kg SO2-eq.","values":[{"value":"2,02E-02","module":"A1-A3","scenario":null},{"value":"1,35E-03","module":"A4","scenario":null},{"value":"8,00E-04","module":"A5","scenario":null},{"value":"0,00E+00","module":"B1","scenario":null},{"value":"1,16E-03","module":"B2","scenario":null},{"value":"7,50E-05","module":"C2","scenario":null},{"value":"4,95E-03","module":"C3","scenario":"S2"},{"value":"5,20E-03","module":"C3","scenario":"S3"},{"value":"9,84E-04","module":"C4","scenario":null},{"value":"-2,18E-05","module":"D","scenario":"S0"},{"value":"0,00E+00","module":"D","scenario":"S1"},{"value":"-3,12E-04","module":"D","scenario":"S2"},{"value":"-9,80E-04","module":"D","scenario":"S3"}]},{"parameter":"EP","unit":"kg PO4^3-eq.","values":[{"value":"1,22E-02","module":"A1-A3","scenario":null},{"value":"3,38E-04","module":"A4","scenario":null},{"value":"4,13E-04","module":"A5","scenario":null},{"value":"0,00E+00","module":"B1","scenario":null},{"value":"3,17E-04","module":"B2","scenario":null},{"value":"1,89E-05","module":"C2","scenario":null},{"value":"1,24E-03","module":"C3","scenario":"S2"},{"value":"1,29E-03","module":"C3","scenario":"S3"},{"value":"1,03E-03","module":"C4","scenario":null},{"value":"-2,73E-06","module":"D","scenario":"S0"},{"value":"0,00E+00","module":"D","scenario":"S1"},{"value":"-3,91E-05","module":"D","scenario":"S2"},{"value":"-1,20E-04","module":"D","scenario":"S3"}]},{"parameter":"POCP","unit":"kg Ethen-eq.","values":[{"value":"1,25E-03","module":"A1-A3","scenario":null},{"value":"-5,66E-04","module":"A4","scenario":null},{"value":"2,83E-05","module":"A5","scenario":null},{"value":"6,29E-05","module":"B1","scenario":null},{"value":"1,48E-04","module":"B2","scenario":null},{"value":"-3,16E-05","module":"C2","scenario":null},{"value":"3,00E-04","module":"C3","scenario":"S2"},{"value":"2,25E-04","module":"C3","scenario":"S3"},{"value":"1,11E-04","module":"C4","scenario":null},{"value":"-2,00E-06","module":"D","scenario":"S0"},{"value":"0,00E+00","module":"D","scenario":"S1"},{"value":"-2,88E-05","module":"D","scenario":"S2"},{"value":"-8,71E-05","module":"D","scenario":"S3"}]},{"parameter":"ADPE","unit":"kg Sb-eq.","values":[{"value":"1,26E-05","module":"A1-A3","scenario":null},{"value":"2,69E-08","module":"A4","scenario":null},{"value":"3,87E-07","module":"A5","scenario":null},{"value":"0,00E+00","module":"B1","scenario":null},{"value":"4,43E-06","module":"B2","scenario":null},{"value":"1,50E-09","module":"C2","scenario":null},{"value":"2,30E-07","module":"C3","scenario":"S2"},{"value":"2,43E-07","module":"C3","scenario":"S3"},{"value":"7,02E-08","module":"C4","scenario":null},{"value":"-3,24E-09","module":"D","scenario":"S0"},{"value":"0,00E+00","module":"D","scenario":"S1"},{"value":"-4,61E-08","module":"D","scenario":"S2"},{"value":"-1,90E-07","module":"D","scenario":"S3"}]},{"parameter":"ADPF","unit":"MJ","values":[{"value":"9,79E+01","module":"A1-A3","scenario":null},{"value":"4,34E+00","module":"A4","scenario":null},{"value":"3,19E+00","module":"A5","scenario":null},{"value":"0,00E+00","module":"B1","scenario":null},{"value":"6,76E+00","module":"B2","scenario":null},{"value":"2,42E-01","module":"C2","scenario":null},{"value":"3,73E+00","module":"C3","scenario":"S2"},{"value":"4,66E+00","module":"C3","scenario":"S3"},{"value":"5,41E+00","module":"C4","scenario":null},{"value":"-2,45E-01","module":"D","scenario":"S0"},{"value":"0,00E+00","module":"D","scenario":"S1"},{"value":"-3,56E+00","module":"D","scenario":"S2"},{"value":"-2,31E+01","module":"D","scenario":"S3"}]}],"additional_environmental_impact":[],"resource_use":[{"parameter":"PERE","unit":"MJ","values":[{"value":"7,10E+01","module":"A1-A3","scenario":null},{"value":"2,45E-01","module":"A4","scenario":null},{"value":"2,90E+00","module":"A5","scenario":null},{"value":"0,00E+00","module":"B1","scenario":null},{"value":"1,20E+00","module":"B2","scenario":null},{"value":"1,37E-02","module":"C2","scenario":null},{"value":"1,39E+01","module":"C3","scenario":"S2"},{"value":"1,41E+01","module":"C3","scenario":"S3"},{"value":"3,92E-01","module":"C4","scenario":null},{"value":"-6,51E-02","module":"D","scenario":"S0"},{"value":"0,00E+00","module":"D","scenario":"S1"},{"value":"-9,21E-01","module":"D","scenario":"S2"},{"value":"-3,45E-01","module":"D","scenario":"S3"}]},{"parameter":"PERM","unit":"MJ","values":[{"value":"1,36E+01","module":"A1-A3","scenario":null},{"value":"0,00E+00","module":"A4","scenario":null},{"value":"-3,39E-01","module":"A5","scenario":null},{"value":"0,00E+00","module":"B1","scenario":null},{"value":"0,00E+00","module":"B2","scenario":null},{"value":"0,00E+00","module":"C2","scenario":null},{"value":"-1,33E+01","module":"C3","scenario":"S2"},{"value":"-1,33E+01","module":"C3","scenario":"S3"},{"value":"0,00E+00","module":"C4","scenario":null},{"value":"0,00E+00","module":"D","scenario":"S0"},{"value":"0,00E+00","module":"D","scenario":"S1"},{"value":"0,00E+00","module":"D","scenario":"S2"},{"value":"0,00E+00","module":"D","scenario":"S3"}]},{"parameter":"PERT","unit":"MJ","values":[{"value":"8,47E+01","module":"A1-A3","scenario":null},{"value":"2,45E-01","module":"A4","scenario":null},{"value":"2,57E+00","module":"A5","scenario":null},{"value":"0,00E+00","module":"B1","scenario":null},{"value":"1,20E+00","module":"B2","scenario":null},{"value":"1,37E-02","module":"C2","scenario":null},{"value":"5,83E-01","module":"C3","scenario":"S2"},{"value":"8,52E-01","module":"C3","scenario":"S3"},{"value":"3,92E-01","module":"C4","scenario":null},{"value":"-6,51E-02","module":"D","scenario":"S0"},{"value":"0,00E+00","module":"D","scenario":"S1"},{"value":"-9,21E-01","module":"D","scenario":"S2"},{"value":"-3,45E-01","module":"D","scenario":"S3"}]},{"parameter":"PENRE","unit":"MJ","values":[{"value":"9,27E+01","module":"A1-A3","scenario":null},{"value":"4,36E+00","module":"A4","scenario":null},{"value":"3,66E+00","module":"A5","scenario":null},{"value":"0,00E+00","module":"B1","scenario":null},{"value":"7,86E+00","module":"B2","scenario":null},{"value":"2,43E-01","module":"C2","scenario":null},{"value":"1,53E+01","module":"C3","scenario":"S2"},{"value":"1,64E+01","module":"C3","scenario":"S3"},{"value":"5,58E+00","module":"C4","scenario":null},{"value":"-3,00E-01","module":"D","scenario":"S0"},{"value":"0,00E+00","module":"D","scenario":"S1"},{"value":"-4,35E+00","module":"D","scenario":"S2"},{"value":"-2,34E+01","module":"D","scenario":"S3"}]},{"parameter":"PENRM","unit":"MJ","values":[{"value":"1,15E+01","module":"A1-A3","scenario":null},{"value":"0,00E+00","module":"A4","scenario":null},{"value":"-2,69E-01","module":"A5","scenario":null},{"value":"0,00E+00","module":"B1","scenario":null},{"value":"0,00E+00","module":"B2","scenario":null},{"value":"0,00E+00","module":"C2","scenario":null},{"value":"-1,12E+01","module":"C3","scenario":"S2"},{"value":"-1,12E+01","module":"C3","scenario":"S3"},{"value":"0,00E+00","module":"C4","scenario":null},{"value":"0,00E+00","module":"D","scenario":"S0"},{"value":"0,00E+00","module":"D","scenario":"S1"},{"value":"0,00E+00","module":"D","scenario":"S2"},{"value":"0,00E+00","module":"D","scenario":"S3"}]},{"parameter":"PENRT","unit":"MJ","values":[{"value":"1,04E+02","module":"A1-A3","scenario":null},{"value":"4,36E+00","module":"A4","scenario":null},{"value":"3,39E+00","module":"A5","scenario":null},{"value":"0,00E+00","module":"B1","scenario":null},{"value":"7,86E+00","module":"B2","scenario":null},{"value":"2,43E-01","module":"C2","scenario":null},{"value":"4,09E+00","module":"C3","scenario":"S2"},{"value":"5,23E+00","module":"C3","scenario":"S3"},{"value":"5,58E+00","module":"C4","scenario":null},{"value":"-3,00E-01","module":"D","scenario":"S0"},{"value":"0,00E+00","module":"D","scenario":"S1"},{"value":"-4,35E+00","module":"D","scenario":"S2"},{"value":"-2,34E+01","module":"D","scenario":"S3"}]},{"parameter":"SM","unit":"kg","values":[{"value":"4,40E+00","module":"A1-A3","scenario":null},{"value":"0,00E+00","module":"A4","scenario":null},{"value":"1,32E-01","module":"A5","scenario":null},{"value":"0,00E+00","module":"B1","scenario":null},{"value":"0,00E+00","module":"B2","scenario":null},{"value":"0,00E+00","module":"C2","scenario":null},{"value":"0,00E+00","module":"C3","scenario":"S2"},{"value":"0,00E+00","module":"C3","scenario":"S3"},{"value":"0,00E+00","module":"C4","scenario":null},{"value":"0,00E+00","module":"D","scenario":"S0"},{"value":"0,00E+00","module":"D","scenario":"S1"},{"value":"0,00E+00","module":"D","scenario":"S2"},{"value":"2,60E-01","module":"D","scenario":"S3"}]},{"parameter":"RSF","unit":"MJ","values":[{"value":"0,00E+00","module":"A1-A3","scenario":null},{"value":"0,00E+00","module":"A4","scenario":null},{"value":"0,00E+00","module":"A5","scenario":null},{"value":"0,00E+00","module":"B1","scenario":null},{"value":"0,00E+00","module":"B2","scenario":null},{"value":"0,00E+00","module":"C2","scenario":null},{"value":"0,00E+00","module":"C3","scenario":"S2"},{"value":"0,00E+00","module":"C3","scenario":"S3"},{"value":"0,00E+00","module":"C4","scenario":null},{"value":"0,00E+00","module":"D","scenario":"S0"},{"value":"0,00E+00","module":"D","scenario":"S1"},{"value":"0,00E+00","module":"D","scenario":"S2"},{"value":"0,00E+00","module":"D","scenario":"S3"}]},{"parameter":"NRSF","unit":"MJ","values":[{"value":"0,00E+00","module":"A1-A3","scenario":null},{"value":"0,00E+00","module":"A4","scenario":null},{"value":"0,00E+00","module":"A5","scenario":null},{"value":"0,00E+00","module":"B1","scenario":null},{"value":"0,00E+00","module":"B2","scenario":null},{"value":"0,00E+00","module":"C2","scenario":null},{"value":"0,00E+00","module":"C3","scenario":"S2"},{"value":"0,00E+00","module":"C3","scenario":"S3"},{"value":"0,00E+00","module":"C4","scenario":null},{"value":"0,00E+00","module":"D","scenario":"S0"},{"value":"0,00E+00","module":"D","scenario":"S1"},{"value":"0,00E+00","module":"D","scenario":"S2"},{"value":"0,00E+00","module":"D","scenario":"S3"}]},{"parameter":"FW","unit":"m^3","values":[{"value":"4,93E-01","module":"A1-A3","scenario":null},{"value":"2,83E-04","module":"A4","scenario":null},{"value":"1,54E-02","module":"A5","scenario":null},{"value":"0,00E+00","module":"B1","scenario":null},{"value":"4,27E-03","module":"B2","scenario":null},{"value":"1,58E-05","module":"C2","scenario":null},{"value":"2,04E-02","module":"C3","scenario":"S2"},{"value":"2,08E-02","module":"C3","scenario":"S3"},{"value":"6,85E-05","module":"C4","scenario":null},{"value":"-7,54E-05","module":"D","scenario":"S0"},{"value":"0,00E+00","module":"D","scenario":"S1"},{"value":"-1,07E-03","module":"D","scenario":"S2"},{"value":"-2,19E-03","module":"D","scenario":"S3"}]}],"end_of_life_waste":[{"parameter":"HWD","unit":"kg","values":[{"value":"6,81E-03","module":"A1-A3","scenario":null},{"value":"2,03E-07","module":"A4","scenario":null},{"value":"2,04E-04","module":"A5","scenario":null},{"value":"0,00E+00","module":"B1","scenario":null},{"value":"9,63E-10","module":"B2","scenario":null},{"value":"1,13E-08","module":"C2","scenario":null},{"value":"1,90E-08","module":"C3","scenario":"S2"},{"value":"4,75E-08","module":"C3","scenario":"S3"},{"value":"2,04E-08","module":"C4","scenario":null},{"value":"-1,20E-10","module":"D","scenario":"S0"},{"value":"0,00E+00","module":"D","scenario":"S1"},{"value":"-1,73E-09","module":"D","scenario":"S2"},{"value":"-5,89E-09","module":"D","scenario":"S3"}]},{"parameter":"NHWD","unit":"kg","values":[{"value":"1,72E+00","module":"A1-A3","scenario":null},{"value":"6,67E-04","module":"A4","scenario":null},{"value":"9,61E-02","module":"A5","scenario":null},{"value":"0,00E+00","module":"B1","scenario":null},{"value":"5,63E-03","module":"B2","scenario":null},{"value":"3,72E-05","module":"C2","scenario":null},{"value":"1,48E+00","module":"C3","scenario":"S2"},{"value":"1,48E+00","module":"C3","scenario":"S3"},{"value":"5,36E+00","module":"C4","scenario":null},{"value":"-1,38E-04","module":"D","scenario":"S0"},{"value":"0,00E+00","module":"D","scenario":"S1"},{"value":"-1,98E-03","module":"D","scenario":"S2"},{"value":"-1,62E-01","module":"D","scenario":"S3"}]},{"parameter":"RWD","unit":"kg","values":[{"value":"2,11E-03","module":"A1-A3","scenario":null},{"value":"5,40E-06","module":"A4","scenario":null},{"value":"6,79E-05","module":"A5","scenario":null},{"value":"0,00E+00","module":"B1","scenario":null},{"value":"3,38E-04","module":"B2","scenario":null},{"value":"3,01E-07","module":"C2","scenario":null},{"value":"1,44E-04","module":"C3","scenario":"S2"},{"value":"2,25E-04","module":"C3","scenario":"S3"},{"value":"6,73E-05","module":"C4","scenario":null},{"value":"-2,22E-05","module":"D","scenario":"S0"},{"value":"0,00E+00","module":"D","scenario":"S1"},{"value":"-3,15E-04","module":"D","scenario":"S2"},{"value":"-8,94E-05","module":"D","scenario":"S3"}]}],"end_of_life_flow":[{"parameter":"CRU","unit":"kg","values":[{"value":"0,00E+00","module":"A1-A3","scenario":null},{"value":"0,00E+00","module":"A4","scenario":null},{"value":"0,00E+00","module":"A5","scenario":null},{"value":"0,00E+00","module":"B1","scenario":null},{"value":"0,00E+00","module":"B2","scenario":null},{"value":"0,00E+00","module":"C2","scenario":null},{"value":"0,00E+00","module":"C3","scenario":"S2"},{"value":"0,00E+00","module":"C3","scenario":"S3"},{"value":"0,00E+00","module":"C4","scenario":null},{"value":"0,00E+00","module":"D","scenario":"S0"},{"value":"0,00E+00","module":"D","scenario":"S1"},{"value":"0,00E+00","module":"D","scenario":"S2"},{"value":"0,00E+00","module":"D","scenario":"S3"}]},{"parameter":"MFR","unit":"kg","values":[{"value":"0,00E+00","module":"A1-A3","scenario":null},{"value":"0,00E+00","module":"A4","scenario":null},{"value":"1,21E-01","module":"A5","scenario":null},{"value":"0,00E+00","module":"B1","scenario":null},{"value":"0,00E+00","module":"B2","scenario":null},{"value":"0,00E+00","module":"C2","scenario":null},{"value":"0,00E+00","module":"C3","scenario":"S2"},{"value":"1,70E+00","module":"C3","scenario":"S3"},{"value":"0,00E+00","module":"C4","scenario":null},{"value":"0,00E+00","module":"D","scenario":"S0"},{"value":"0,00E+00","module":"D","scenario":"S1"},{"value":"0,00E+00","module":"D","scenario":"S2"},{"value":"0,00E+00","module":"D","scenario":"S3"}]},{"parameter":"MER","unit":"kg","values":[{"value":"0,00E+00","module":"A1-A3","scenario":null},{"value":"0,00E+00","module":"A4","scenario":null},{"value":"0,00E+00","module":"A5","scenario":null},{"value":"0,00E+00","module":"B1","scenario":null},{"value":"0,00E+00","module":"B2","scenario":null},{"value":"0,00E+00","module":"C2","scenario":null},{"value":"0,00E+00","module":"C3","scenario":"S2"},{"value":"0,00E+00","module":"C3","scenario":"S3"},{"value":"0,00E+00","module":"C4","scenario":null},{"value":"0,00E+00","module":"D","scenario":"S0"},{"value":"0,00E+00","module":"D","scenario":"S1"},{"value":"0,00E+00","module":"D","scenario":"S2"},{"value":"0,00E+00","module":"D","scenario":"S3"}]},{"parameter":"EEE","unit":"MJ","values":[{"value":"0,00E+00","module":"A1-A3","scenario":null},{"value":"0,00E+00","module":"A4","scenario":null},{"value":"2,79E-01","module":"A5","scenario":null},{"value":"0,00E+00","module":"B1","scenario":null},{"value":"0,00E+00","module":"B2","scenario":null},{"value":"0,00E+00","module":"C2","scenario":null},{"value":"7,88E+00","module":"C3","scenario":"S2"},{"value":"0,00E+00","module":"C3","scenario":"S3"},{"value":"0,00E+00","module":"C4","scenario":null},{"value":"0,00E+00","module":"D","scenario":"S0"},{"value":"0,00E+00","module":"D","scenario":"S1"},{"value":"0,00E+00","module":"D","scenario":"S2"},{"value":"0,00E+00","module":"D","scenario":"S3"}]},{"parameter":"EET","unit":"MJ","values":[{"value":"0,00E+00","module":"A1-A3","scenario":null},{"value":"0,00E+00","module":"A4","scenario":null},{"value":"5,18E-01","module":"A5","scenario":null},{"value":"0,00E+00","module":"B1","scenario":null},{"value":"0,00E+00","module":"B2","scenario":null},{"value":"0,00E+00","module":"C2","scenario":null},{"value":"1,47E+01","module":"C3","scenario":"S2"},{"value":"8,41E+01","module":"C3","scenario":"S3"},{"value":"0,00E+00","module":"C4","scenario":null},{"value":"0,00E+00","module":"D","scenario":"S0"},{"value":"0,00E+00","module":"D","scenario":"S1"},{"value":"0,00E+00","module":"D","scenario":"S2"},{"value":"0,00E+00","module":"D","scenario":"S3"}]}]}