{
    "product_name": "Elektromechanische Schl\u00f6sser, Beschl\u00e4ge und Dreht\u00fcrantriebe",
    "epd_id": "EPD-ARG-20230552-IBG3-EN",
    "compliance": [
        "DIN EN 15804+A2",
        "ISO 14025"
    ],
    "producer_name": "ARGE \u2013 The European Federation of Locks and Building Hardware Manufacturers",
    "environmental_impact": [
        {
            "parameter": "GWP-total",
            "values": [
                {
                    "value": "1,18E+01",
                    "module": "A1-A3",
                    "scenario": null
                },
                {
                    "value": "6,75E-01",
                    "module": "A4",
                    "scenario": null
                },
                {
                    "value": "3,14E-01",
                    "module": "A5",
                    "scenario": null
                },
                {
                    "value": "1,48E+00",
                    "module": "B6",
                    "scenario": "S1"
                },
                {
                    "value": "2,03E+02",
                    "module": "B6",
                    "scenario": "S2"
                },
                {
                    "value": "0,00E+00",
                    "module": "C1",
                    "scenario": null
                },
                {
                    "value": "1,86E-02",
                    "module": "C2",
                    "scenario": null
                },
                {
                    "value": "1,86E-02",
                    "module": "C3",
                    "scenario": null
                },
                {
                    "value": "4,93E-02",
                    "module": "C4",
                    "scenario": null
                },
                {
                    "value": "4,85E-01",
                    "module": "D",
                    "scenario": null
                }
            ]
        },
        {
            "parameter": "GWP-fossil",
            "values": [
                {
                    "value": "1,20E+01",
                    "module": "A1-A3",
                    "scenario": null
                },
                {
                    "value": "6,74E-01",
                    "module": "A4",
                    "scenario": null
                },
                {
                    "value": "2,26E-02",
                    "module": "A5",
                    "scenario": null
                },
                {
                    "value": "1,47E+00",
                    "module": "B6",
                    "scenario": "S1"
                },
                {
                    "value": "2,03E+02",
                    "module": "B6",
                    "scenario": "S2"
                },
                {
                    "value": "0,00E+00",
                    "module": "C1",
                    "scenario": null
                },
                {
                    "value": "1,86E-02",
                    "module": "C2",
                    "scenario": null
                },
                {
                    "value": "1,85E-02",
                    "module": "C3",
                    "scenario": null
                },
                {
                    "value": "4,93E-02",
                    "module": "C4",
                    "scenario": null
                },
                {
                    "value": "4,84E-01",
                    "module": "D",
                    "scenario": null
                }
            ]
        },
        {
            "parameter": "GWP-biogenic",
            "values": [
                {
                    "value": "-2,69E-01",
                    "module": "A1-A3",
                    "scenario": null
                },
                {
                    "value": "0,00E+00",
                    "module": "A4",
                    "scenario": null
                },
                {
                    "value": "2,92E-01",
                    "module": "A5",
                    "scenario": null
                },
                {
                    "value": "0,00E+00",
                    "module": "B6",
                    "scenario": "S1"
                },
                {
                    "value": "0,00E+00",
                    "module": "B6",
                    "scenario": "S2"
                },
                {
                    "value": "0,00E+00",
                    "module": "C1",
                    "scenario": null
                },
                {
                    "value": "0,00E+00",
                    "module": "C2",
                    "scenario": null
                },
                {
                    "value": "0,00E+00",
                    "module": "C3",
                    "scenario": null
                },
                {
                    "value": "0,00E+00",
                    "module": "C4",
                    "scenario": null
                },
                {
                    "value": "0,00E+00",
                    "module": "D",
                    "scenario": null
                }
            ]
        },
        {
            "parameter": "GWP-luluc",
            "values": [
                {
                    "value": "2,82E-02",
                    "module": "A1-A3",
                    "scenario": null
                },
                {
                    "value": "2,70E-04",
                    "module": "A4",
                    "scenario": null
                },
                {
                    "value": "1,80E-06",
                    "module": "A5",
                    "scenario": null
                },
                {
                    "value": "2,69E-03",
                    "module": "B6",
                    "scenario": "S1"
                },
                {
                    "value": "5,07E-01",
                    "module": "B6",
                    "scenario": "S2"
                },
                {
                    "value": "0,00E+00",
                    "module": "C1",
                    "scenario": null
                },
                {
                    "value": "7,44E-06",
                    "module": "C2",
                    "scenario": null
                },
                {
                    "value": "3,14E-05",
                    "module": "C3",
                    "scenario": null
                },
                {
                    "value": "3,75E-06",
                    "module": "C4",
                    "scenario": null
                },
                {
                    "value": "7,47E-04",
                    "module": "D",
                    "scenario": null
                }
            ]
        },
        {
            "parameter": "ODP",
            "values": [
                {
                    "value": "6,48E-07",
                    "module": "A1-A3",
                    "scenario": null
                },
                {
                    "value": "1,56E-07",
                    "module": "A4",
                    "scenario": null
                },
                {
                    "value": "1,02E-09",
                    "module": "A5",
                    "scenario": null
                },
                {
                    "value": "1,15E-07",
                    "module": "B6",
                    "scenario": "S1"
                },
                {
                    "value": "1,05E-05",
                    "module": "B6",
                    "scenario": "S2"
                },
                {
                    "value": "0,00E+00",
                    "module": "C1",
                    "scenario": null
                },
                {
                    "value": "4,31E-09",
                    "module": "C2",
                    "scenario": null
                },
                {
                    "value": "8,96E-10",
                    "module": "C3",
                    "scenario": null
                },
                {
                    "value": "1,52E-09",
                    "module": "C4",
                    "scenario": null
                },
                {
                    "value": "3,20E-08",
                    "module": "D",
                    "scenario": null
                }
            ]
        },
        {
            "parameter": "AP",
            "values": [
                {
                    "value": "3,08E-01",
                    "module": "A1-A3",
                    "scenario": null
                },
                {
                    "value": "1,91E-03",
                    "module": "A4",
                    "scenario": null
                },
                {
                    "value": "1,95E-05",
                    "module": "A5",
                    "scenario": null
                },
                {
                    "value": "3,07E-02",
                    "module": "B6",
                    "scenario": "S1"
                },
                {
                    "value": "1,11E+00",
                    "module": "B6",
                    "scenario": "S2"
                },
                {
                    "value": "0,00E+00",
                    "module": "C1",
                    "scenario": null
                },
                {
                    "value": "5,28E-05",
                    "module": "C2",
                    "scenario": null
                },
                {
                    "value": "2,03E-04",
                    "module": "C3",
                    "scenario": null
                },
                {
                    "value": "4,35E-05",
                    "module": "C4",
                    "scenario": null
                },
                {
                    "value": "2,35E-02",
                    "module": "D",
                    "scenario": null
                }
            ]
        },
        {
            "parameter": "POCP",
            "values": [
                {
                    "value": "7,77E-02",
                    "module": "A1-A3",
                    "scenario": null
                },
                {
                    "value": "1,63E-03",
                    "module": "A4",
                    "scenario": null
                },
                {
                    "value": "2,03E-05",
                    "module": "A5",
                    "scenario": null
                },
                {
                    "value": "8,53E-03",
                    "module": "B6",
                    "scenario": "S1"
                },
                {
                    "value": "4,40E-01",
                    "module": "B6",
                    "scenario": "S2"
                },
                {
                    "value": "0,00E+00",
                    "module": "C1",
                    "scenario": null
                },
                {
                    "value": "4,50E-05",
                    "module": "C2",
                    "scenario": null
                },
                {
                    "value": "5,78E-05",
                    "module": "C3",
                    "scenario": null
                },
                {
                    "value": "4,98E-05",
                    "module": "C4",
                    "scenario": null
                },
                {
                    "value": "4,23E-03",
                    "module": "D",
                    "scenario": null
                }
            ]
        },
        {
            "parameter": "ADPE",
            "values": [
                {
                    "value": "4,07E-03",
                    "module": "A1-A3",
                    "scenario": null
                },
                {
                    "value": "2,39E-06",
                    "module": "A4",
                    "scenario": null
                },
                {
                    "value": "1,62E-08",
                    "module": "A5",
                    "scenario": null
                },
                {
                    "value": "5,70E-04",
                    "module": "B6",
                    "scenario": "S1"
                },
                {
                    "value": "1,97E-03",
                    "module": "B6",
                    "scenario": "S2"
                },
                {
                    "value": "0,00E+00",
                    "module": "C1",
                    "scenario": null
                },
                {
                    "value": "6,59E-08",
                    "module": "C2",
                    "scenario": null
                },
                {
                    "value": "7,78E-07",
                    "module": "C3",
                    "scenario": null
                },
                {
                    "value": "2,26E-08",
                    "module": "C4",
                    "scenario": null
                },
                {
                    "value": "5,66E-04",
                    "module": "D",
                    "scenario": null
                }
            ]
        },
        {
            "parameter": "ADPF",
            "values": [
                {
                    "value": "1,29E+02",
                    "module": "A1-A3",
                    "scenario": null
                },
                {
                    "value": "1,02E+01",
                    "module": "A4",
                    "scenario": null
                },
                {
                    "value": "6,85E-02",
                    "module": "A5",
                    "scenario": null
                },
                {
                    "value": "1,93E+01",
                    "module": "B6",
                    "scenario": "S1"
                },
                {
                    "value": "4,27E+03",
                    "module": "B6",
                    "scenario": "S2"
                },
                {
                    "value": "0,00E+00",
                    "module": "C1",
                    "scenario": null
                },
                {
                    "value": "2,82E-01",
                    "module": "C2",
                    "scenario": null
                },
                {
                    "value": "2,38E-01",
                    "module": "C3",
                    "scenario": null
                },
                {
                    "value": "1,11E-01",
                    "module": "C4",
                    "scenario": null
                },
                {
                    "value": "6,82E+00",
                    "module": "D",
                    "scenario": null
                }
            ]
        },
        {
            "parameter": "WDP",
            "values": [
                {
                    "value": "5,06E+00",
                    "module": "A1-A3",
                    "scenario": null
                },
                {
                    "value": "3,11E-02",
                    "module": "A4",
                    "scenario": null
                },
                {
                    "value": "3,36E-04",
                    "module": "A5",
                    "scenario": null
                },
                {
                    "value": "8,35E-01",
                    "module": "B6",
                    "scenario": "S1"
                },
                {
                    "value": "5,07E+01",
                    "module": "B6",
                    "scenario": "S2"
                },
                {
                    "value": "0,00E+00",
                    "module": "C1",
                    "scenario": null
                },
                {
                    "value": "8,58E-04",
                    "module": "C2",
                    "scenario": null
                },
                {
                    "value": "9,87E-03",
                    "module": "C3",
                    "scenario": null
                },
                {
                    "value": "-3,16E-04",
                    "module": "C4",
                    "scenario": null
                },
                {
                    "value": "4,14E-01",
                    "module": "D",
                    "scenario": null
                }
            ]
        },
        {
            "parameter": "EP-freshwater",
            "values": [
                {
                    "value": "1,87E-03",
                    "module": "A1-A3",
                    "scenario": null
                },
                {
                    "value": "4,81E-06",
                    "module": "A4",
                    "scenario": null
                },
                {
                    "value": "3,74E-08",
                    "module": "A5",
                    "scenario": null
                },
                {
                    "value": "1,66E-04",
                    "module": "B6",
                    "scenario": "S1"
                },
                {
                    "value": "2,27E-02",
                    "module": "B6",
                    "scenario": "S2"
                },
                {
                    "value": "0,00E+00",
                    "module": "C1",
                    "scenario": null
                },
                {
                    "value": "1,33E-07",
                    "module": "C2",
                    "scenario": null
                },
                {
                    "value": "1,06E-06",
                    "module": "C3",
                    "scenario": null
                },
                {
                    "value": "8,24E-08",
                    "module": "C4",
                    "scenario": null
                },
                {
                    "value": "7,47E-05",
                    "module": "D",
                    "scenario": null
                }
            ]
        },
        {
            "parameter": "EP-marine",
            "values": [
                {
                    "value": "3,85E-02",
                    "module": "A1-A3",
                    "scenario": null
                },
                {
                    "value": "3,81E-04",
                    "module": "A4",
                    "scenario": null
                },
                {
                    "value": "6,46E-06",
                    "module": "A5",
                    "scenario": null
                },
                {
                    "value": "2,35E-03",
                    "module": "B6",
                    "scenario": "S1"
                },
                {
                    "value": "1,38E-01",
                    "module": "B6",
                    "scenario": "S2"
                },
                {
                    "value": "0,00E+00",
                    "module": "C1",
                    "scenario": null
                },
                {
                    "value": "1,05E-05",
                    "module": "C2",
                    "scenario": null
                },
                {
                    "value": "1,67E-05",
                    "module": "C3",
                    "scenario": null
                },
                {
                    "value": "1,76E-05",
                    "module": "C4",
                    "scenario": null
                },
                {
                    "value": "1,02E-03",
                    "module": "D",
                    "scenario": null
                }
            ]
        },
        {
            "parameter": "EP-terrestrial",
            "values": [
                {
                    "value": "2,80E-01",
                    "module": "A1-A3",
                    "scenario": null
                },
                {
                    "value": "4,24E-03",
                    "module": "A4",
                    "scenario": null
                },
                {
                    "value": "6,99E-05",
                    "module": "A5",
                    "scenario": null
                },
                {
                    "value": "2,81E-02",
                    "module": "B6",
                    "scenario": "S1"
                },
                {
                    "value": "1,60E+00",
                    "module": "B6",
                    "scenario": "S2"
                },
                {
                    "value": "0,00E+00",
                    "module": "C1",
                    "scenario": null
                },
                {
                    "value": "1,17E-04",
                    "module": "C2",
                    "scenario": null
                },
                {
                    "value": "1,85E-04",
                    "module": "C3",
                    "scenario": null
                },
                {
                    "value": "1,70E-04",
                    "module": "C4",
                    "scenario": null
                },
                {
                    "value": "1,40E-02",
                    "module": "D",
                    "scenario": null
                }
            ]
        }
    ],
    "additional_environmental_impact": [
        {
            "parameter": "PM",
            "values": [
                {
                    "value": "1,29E-06",
                    "module": "A1-A3",
                    "scenario": null
                },
                {
                    "value": "5,42E-08",
                    "module": "A4",
                    "scenario": null
                },
                {
                    "value": "3,98E-10",
                    "module": "A5",
                    "scenario": null
                },
                {
                    "value": "1,34E-07",
                    "module": "B6",
                    "scenario": "S1"
                },
                {
                    "value": "3,24E-06",
                    "module": "B6",
                    "scenario": "S2"
                },
                {
                    "value": "0,00E+00",
                    "module": "C1",
                    "scenario": null
                },
                {
                    "value": "1,49E-09",
                    "module": "C2",
                    "scenario": null
                },
                {
                    "value": "1,19E-09",
                    "module": "C3",
                    "scenario": null
                },
                {
                    "value": "1,05E-09",
                    "module": "C4",
                    "scenario": null
                },
                {
                    "value": "5,38E-08",
                    "module": "D",
                    "scenario": null
                }
            ]
        },
        {
            "parameter": "ETP-fw",
            "values": [
                {
                    "value": "2,54E+03",
                    "module": "A1-A3",
                    "scenario": null
                },
                {
                    "value": "8,02E+00",
                    "module": "A4",
                    "scenario": null
                },
                {
                    "value": "5,87E-02",
                    "module": "A5",
                    "scenario": null
                },
                {
                    "value": "2,18E+02",
                    "module": "B6",
                    "scenario": "S1"
                },
                {
                    "value": "2,67E+03",
                    "module": "B6",
                    "scenario": "S2"
                },
                {
                    "value": "0,00E+00",
                    "module": "C1",
                    "scenario": null
                },
                {
                    "value": "2,21E-01",
                    "module": "C2",
                    "scenario": null
                },
                {
                    "value": "1,06E+00",
                    "module": "C3",
                    "scenario": null
                },
                {
                    "value": "5,48E+01",
                    "module": "C4",
                    "scenario": null
                },
                {
                    "value": "1,28E+02",
                    "module": "D",
                    "scenario": null
                }
            ]
        },
        {
            "parameter": "HTP-c",
            "values": [
                {
                    "value": "6,79E-08",
                    "module": "A1-A3",
                    "scenario": null
                },
                {
                    "value": "2,58E-10",
                    "module": "A4",
                    "scenario": null
                },
                {
                    "value": "3,64E-12",
                    "module": "A5",
                    "scenario": null
                },
                {
                    "value": "8,96E-09",
                    "module": "B6",
                    "scenario": "S1"
                },
                {
                    "value": "8,58E-08",
                    "module": "B6",
                    "scenario": "S2"
                },
                {
                    "value": "0,00E+00",
                    "module": "C1",
                    "scenario": null
                },
                {
                    "value": "7,12E-12",
                    "module": "C2",
                    "scenario": null
                },
                {
                    "value": "2,13E-11",
                    "module": "C3",
                    "scenario": null
                },
                {
                    "value": "1,22E-11",
                    "module": "C4",
                    "scenario": null
                },
                {
                    "value": "5,60E-09",
                    "module": "D",
                    "scenario": null
                }
            ]
        },
        {
            "parameter": "HTP-nc",
            "values": [
                {
                    "value": "3,43E-06",
                    "module": "A1-A3",
                    "scenario": null
                },
                {
                    "value": "8,11E-09",
                    "module": "A4",
                    "scenario": null
                },
                {
                    "value": "1,44E-10",
                    "module": "A5",
                    "scenario": null
                },
                {
                    "value": "3,53E-07",
                    "module": "B6",
                    "scenario": "S1"
                },
                {
                    "value": "2,70E-06",
                    "module": "B6",
                    "scenario": "S2"
                },
                {
                    "value": "0,00E+00",
                    "module": "C1",
                    "scenario": null
                },
                {
                    "value": "2,24E-10",
                    "module": "C2",
                    "scenario": null
                },
                {
                    "value": "5,82E-10",
                    "module": "C3",
                    "scenario": null
                },
                {
                    "value": "3,96E-10",
                    "module": "C4",
                    "scenario": null
                },
                {
                    "value": "3,81E-07",
                    "module": "D",
                    "scenario": null
                }
            ]
        },
        {
            "parameter": "SQP",
            "values": [
                {
                    "value": "1,14E+02",
                    "module": "A1-A3",
                    "scenario": null
                },
                {
                    "value": "7,13E+00",
                    "module": "A4",
                    "scenario": null
                },
                {
                    "value": "4,58E-02",
                    "module": "A5",
                    "scenario": null
                },
                {
                    "value": "1,12E+01",
                    "module": "B6",
                    "scenario": "S1"
                },
                {
                    "value": "8,22E+02",
                    "module": "B6",
                    "scenario": "S2"
                },
                {
                    "value": "0,00E+00",
                    "module": "C1",
                    "scenario": null
                },
                {
                    "value": "1,96E-01",
                    "module": "C2",
                    "scenario": null
                },
                {
                    "value": "7,52E-02",
                    "module": "C3",
                    "scenario": null
                },
                {
                    "value": "1,89E-01",
                    "module": "C4",
                    "scenario": null
                },
                {
                    "value": "8,77E+00",
                    "module": "D",
                    "scenario": null
                }
            ]
        }
    ],
    "resource_use": [
        {
            "parameter": "PERE",
            "values": [
                {
                    "value": "2,15E+01",
                    "module": "A1-A3",
                    "scenario": null
                },
                {
                    "value": "1,44E-01",
                    "module": "A4",
                    "scenario": null
                },
                {
                    "value": "-6,86E-01",
                    "module": "A5",
                    "scenario": null
                },
                {
                    "value": "2,56E+00",
                    "module": "B6",
                    "scenario": "S1"
                },
                {
                    "value": "9,42E+02",
                    "module": "B6",
                    "scenario": "S2"
                },
                {
                    "value": "0,00E+00",
                    "module": "C1",
                    "scenario": null
                },
                {
                    "value": "3,96E-03",
                    "module": "C2",
                    "scenario": null
                },
                {
                    "value": "9,18E-02",
                    "module": "C3",
                    "scenario": null
                },
                {
                    "value": "6,71E-03",
                    "module": "C4",
                    "scenario": null
                },
                {
                    "value": "1,33E+00",
                    "module": "D",
                    "scenario": null
                }
            ]
        },
        {
            "parameter": "PERM",
            "values": [
                {
                    "value": "2,35E+00",
                    "module": "A1-A3",
                    "scenario": null
                },
                {
                    "value": "0,00E+00",
                    "module": "A4",
                    "scenario": null
                },
                {
                    "value": "-6,18E-01",
                    "module": "A5",
                    "scenario": null
                },
                {
                    "value": "0,00E+00",
                    "module": "B6",
                    "scenario": "S1"
                },
                {
                    "value": "0,00E+00",
                    "module": "B6",
                    "scenario": "S2"
                },
                {
                    "value": "0,00E+00",
                    "module": "C1",
                    "scenario": null
                },
                {
                    "value": "0,00E+00",
                    "module": "C2",
                    "scenario": null
                },
                {
                    "value": "0,00E+00",
                    "module": "C3",
                    "scenario": null
                },
                {
                    "value": "0,00E+00",
                    "module": "C4",
                    "scenario": null
                },
                {
                    "value": "0,00E+00",
                    "module": "D",
                    "scenario": null
                }
            ]
        },
        {
            "parameter": "PERT",
            "values": [
                {
                    "value": "2,38E+01",
                    "module": "A1-A3",
                    "scenario": null
                },
                {
                    "value": "1,44E-01",
                    "module": "A4",
                    "scenario": null
                },
                {
                    "value": "-1,30E+00",
                    "module": "A5",
                    "scenario": null
                },
                {
                    "value": "2,56E+00",
                    "module": "B6",
                    "scenario": "S1"
                },
                {
                    "value": "9,42E+02",
                    "module": "B6",
                    "scenario": "S2"
                },
                {
                    "value": "0,00E+00",
                    "module": "C1",
                    "scenario": null
                },
                {
                    "value": "3,96E-03",
                    "module": "C2",
                    "scenario": null
                },
                {
                    "value": "9,18E-02",
                    "module": "C3",
                    "scenario": null
                },
                {
                    "value": "6,71E-03",
                    "module": "C4",
                    "scenario": null
                },
                {
                    "value": "1,33E+00",
                    "module": "D",
                    "scenario": null
                }
            ]
        },
        {
            "parameter": "PENRE",
            "values": [
                {
                    "value": "1,31E+02",
                    "module": "A1-A3",
                    "scenario": null
                },
                {
                    "value": "1,02E+01",
                    "module": "A4",
                    "scenario": null
                },
                {
                    "value": "2,17E-01",
                    "module": "A5",
                    "scenario": null
                },
                {
                    "value": "1,93E+01",
                    "module": "B6",
                    "scenario": "S1"
                },
                {
                    "value": "4,32E+03",
                    "module": "B6",
                    "scenario": "S2"
                },
                {
                    "value": "0,00E+00",
                    "module": "C1",
                    "scenario": null
                },
                {
                    "value": "2,82E-01",
                    "module": "C2",
                    "scenario": null
                },
                {
                    "value": "2,39E-01",
                    "module": "C3",
                    "scenario": null
                },
                {
                    "value": "1,11E-01",
                    "module": "C4",
                    "scenario": null
                },
                {
                    "value": "6,85E+00",
                    "module": "D",
                    "scenario": null
                }
            ]
        },
        {
            "parameter": "PENRM",
            "values": [
                {
                    "value": "1,43E+00",
                    "module": "A1-A3",
                    "scenario": null
                },
                {
                    "value": "0,00E+00",
                    "module": "A4",
                    "scenario": null
                },
                {
                    "value": "-1,48E-01",
                    "module": "A5",
                    "scenario": null
                },
                {
                    "value": "0,00E+00",
                    "module": "B6",
                    "scenario": "S1"
                },
                {
                    "value": "0,00E+00",
                    "module": "B6",
                    "scenario": "S2"
                },
                {
                    "value": "0,00E+00",
                    "module": "C1",
                    "scenario": null
                },
                {
                    "value": "0,00E+00",
                    "module": "C2",
                    "scenario": null
                },
                {
                    "value": "0,00E+00",
                    "module": "C3",
                    "scenario": null
                },
                {
                    "value": "0,00E+00",
                    "module": "C4",
                    "scenario": null
                },
                {
                    "value": "0,00E+00",
                    "module": "D",
                    "scenario": null
                }
            ]
        },
        {
            "parameter": "PENRT",
            "values": [
                {
                    "value": "1,33E+02",
                    "module": "A1-A3",
                    "scenario": null
                },
                {
                    "value": "1,02E+01",
                    "module": "A4",
                    "scenario": null
                },
                {
                    "value": "6,85E-02",
                    "module": "A5",
                    "scenario": null
                },
                {
                    "value": "1,93E+01",
                    "module": "B6",
                    "scenario": "S1"
                },
                {
                    "value": "4,32E+03",
                    "module": "B6",
                    "scenario": "S2"
                },
                {
                    "value": "0,00E+00",
                    "module": "C1",
                    "scenario": null
                },
                {
                    "value": "2,82E-01",
                    "module": "C2",
                    "scenario": null
                },
                {
                    "value": "2,39E-01",
                    "module": "C3",
                    "scenario": null
                },
                {
                    "value": "1,11E-01",
                    "module": "C4",
                    "scenario": null
                },
                {
                    "value": "6,85E+00",
                    "module": "D",
                    "scenario": null
                }
            ]
        },
        {
            "parameter": "SM",
            "values": [
                {
                    "value": "4,47E-01",
                    "module": "A1-A3",
                    "scenario": null
                },
                {
                    "value": "0,00E+00",
                    "module": "A4",
                    "scenario": null
                },
                {
                    "value": "0,00E+00",
                    "module": "A5",
                    "scenario": null
                },
                {
                    "value": "0,00E+00",
                    "module": "B6",
                    "scenario": "S1"
                },
                {
                    "value": "0,00E+00",
                    "module": "B6",
                    "scenario": "S2"
                },
                {
                    "value": "0,00E+00",
                    "module": "C1",
                    "scenario": null
                },
                {
                    "value": "0,00E+00",
                    "module": "C2",
                    "scenario": null
                },
                {
                    "value": "0,00E+00",
                    "module": "C3",
                    "scenario": null
                },
                {
                    "value": "0,00E+00",
                    "module": "C4",
                    "scenario": null
                },
                {
                    "value": "0,00E+00",
                    "module": "D",
                    "scenario": null
                }
            ]
        },
        {
            "parameter": "RSF",
            "values": [
                {
                    "value": "0,00E+00",
                    "module": "A1-A3",
                    "scenario": null
                },
                {
                    "value": "0,00E+00",
                    "module": "A4",
                    "scenario": null
                },
                {
                    "value": "0,00E+00",
                    "module": "A5",
                    "scenario": null
                },
                {
                    "value": "0,00E+00",
                    "module": "B6",
                    "scenario": "S1"
                },
                {
                    "value": "0,00E+00",
                    "module": "B6",
                    "scenario": "S2"
                },
                {
                    "value": "0,00E+00",
                    "module": "C1",
                    "scenario": null
                },
                {
                    "value": "0,00E+00",
                    "module": "C2",
                    "scenario": null
                },
                {
                    "value": "0,00E+00",
                    "module": "C3",
                    "scenario": null
                },
                {
                    "value": "0,00E+00",
                    "module": "C4",
                    "scenario": null
                },
                {
                    "value": "0,00E+00",
                    "module": "D",
                    "scenario": null
                }
            ]
        },
        {
            "parameter": "NRSF",
            "values": [
                {
                    "value": "0,00E+00",
                    "module": "A1-A3",
                    "scenario": null
                },
                {
                    "value": "0,00E+00",
                    "module": "A4",
                    "scenario": null
                },
                {
                    "value": "0,00E+00",
                    "module": "A5",
                    "scenario": null
                },
                {
                    "value": "0,00E+00",
                    "module": "B6",
                    "scenario": "S1"
                },
                {
                    "value": "0,00E+00",
                    "module": "B6",
                    "scenario": "S2"
                },
                {
                    "value": "0,00E+00",
                    "module": "C1",
                    "scenario": null
                },
                {
                    "value": "0,00E+00",
                    "module": "C2",
                    "scenario": null
                },
                {
                    "value": "0,00E+00",
                    "module": "C3",
                    "scenario": null
                },
                {
                    "value": "0,00E+00",
                    "module": "C4",
                    "scenario": null
                },
                {
                    "value": "0,00E+00",
                    "module": "D",
                    "scenario": null
                }
            ]
        },
        {
            "parameter": "FW",
            "values": [
                {
                    "value": "1,62E-01",
                    "module": "A1-A3",
                    "scenario": null
                },
                {
                    "value": "1,08E-03",
                    "module": "A4",
                    "scenario": null
                },
                {
                    "value": "5,13E-05",
                    "module": "A5",
                    "scenario": null
                },
                {
                    "value": "1,88E-02",
                    "module": "B6",
                    "scenario": "S1"
                },
                {
                    "value": "2,84E+00",
                    "module": "B6",
                    "scenario": "S2"
                },
                {
                    "value": "0,00E+00",
                    "module": "C1",
                    "scenario": null
                },
                {
                    "value": "2,99E-05",
                    "module": "C2",
                    "scenario": null
                },
                {
                    "value": "2,75E-04",
                    "module": "C3",
                    "scenario": null
                },
                {
                    "value": "2,23E-04",
                    "module": "C4",
                    "scenario": null
                },
                {
                    "value": "6,66E-03",
                    "module": "D",
                    "scenario": null
                }
            ]
        }
    ],
    "end_of_life_waste": [
        {
            "parameter": "HWD",
            "values": [
                {
                    "value": "1,47E-03",
                    "module": "A1-A3",
                    "scenario": null
                },
                {
                    "value": "2,67E-05",
                    "module": "A4",
                    "scenario": null
                },
                {
                    "value": "2,49E-07",
                    "module": "A5",
                    "scenario": null
                },
                {
                    "value": "7,99E-04",
                    "module": "B6",
                    "scenario": "S1"
                },
                {
                    "value": "3,41E-03",
                    "module": "B6",
                    "scenario": "S2"
                },
                {
                    "value": "0,00E+00",
                    "module": "C1",
                    "scenario": null
                },
                {
                    "value": "7,36E-07",
                    "module": "C2",
                    "scenario": null
                },
                {
                    "value": "4,47E-07",
                    "module": "C3",
                    "scenario": null
                },
                {
                    "value": "2,15E-07",
                    "module": "C4",
                    "scenario": null
                },
                {
                    "value": "1,92E-04",
                    "module": "D",
                    "scenario": null
                }
            ]
        },
        {
            "parameter": "NHWD",
            "values": [
                {
                    "value": "4,71E+00",
                    "module": "A1-A3",
                    "scenario": null
                },
                {
                    "value": "5,38E-01",
                    "module": "A4",
                    "scenario": null
                },
                {
                    "value": "4,05E-03",
                    "module": "A5",
                    "scenario": null
                },
                {
                    "value": "5,53E-01",
                    "module": "B6",
                    "scenario": "S1"
                },
                {
                    "value": "1,72E+01",
                    "module": "B6",
                    "scenario": "S2"
                },
                {
                    "value": "0,00E+00",
                    "module": "C1",
                    "scenario": null
                },
                {
                    "value": "1,48E-02",
                    "module": "C2",
                    "scenario": null
                },
                {
                    "value": "1,37E-02",
                    "module": "C3",
                    "scenario": null
                },
                {
                    "value": "3,80E-01",
                    "module": "C4",
                    "scenario": null
                },
                {
                    "value": "1,71E-01",
                    "module": "D",
                    "scenario": null
                }
            ]
        },
        {
            "parameter": "RWD",
            "values": [
                {
                    "value": "2,12E-03",
                    "module": "A1-A3",
                    "scenario": null
                },
                {
                    "value": "1,48E-04",
                    "module": "A4",
                    "scenario": null
                },
                {
                    "value": "9,43E-07",
                    "module": "A5",
                    "scenario": null
                },
                {
                    "value": "9,02E-05",
                    "module": "B6",
                    "scenario": "S1"
                },
                {
                    "value": "5,73E-02",
                    "module": "B6",
                    "scenario": "S2"
                },
                {
                    "value": "0,00E+00",
                    "module": "C1",
                    "scenario": null
                },
                {
                    "value": "4,08E-06",
                    "module": "C2",
                    "scenario": null
                },
                {
                    "value": "1,95E-06",
                    "module": "C3",
                    "scenario": null
                },
                {
                    "value": "1,41E-06",
                    "module": "C4",
                    "scenario": null
                },
                {
                    "value": "5,49E-05",
                    "module": "D",
                    "scenario": null
                }
            ]
        }
    ],
    "end_of_life_flow": [
        {
            "parameter": "CRU",
            "values": [
                {
                    "value": "0,00E+00",
                    "module": "A1-A3",
                    "scenario": null
                },
                {
                    "value": "0,00E+00",
                    "module": "A4",
                    "scenario": null
                },
                {
                    "value": "0,00E+00",
                    "module": "A5",
                    "scenario": null
                },
                {
                    "value": "0,00E+00",
                    "module": "B6",
                    "scenario": "S1"
                },
                {
                    "value": "0,00E+00",
                    "module": "B6",
                    "scenario": "S2"
                },
                {
                    "value": "0,00E+00",
                    "module": "C1",
                    "scenario": null
                },
                {
                    "value": "0,00E+00",
                    "module": "C2",
                    "scenario": null
                },
                {
                    "value": "0,00E+00",
                    "module": "C3",
                    "scenario": null
                },
                {
                    "value": "0,00E+00",
                    "module": "C4",
                    "scenario": null
                },
                {
                    "value": "0,00E+00",
                    "module": "D",
                    "scenario": null
                }
            ]
        },
        {
            "parameter": "MFR",
            "values": [
                {
                    "value": "2,89E-01",
                    "module": "A1-A3",
                    "scenario": null
                },
                {
                    "value": "0,00E+00",
                    "module": "A4",
                    "scenario": null
                },
                {
                    "value": "1,61E-01",
                    "module": "A5",
                    "scenario": null
                },
                {
                    "value": "0,00E+00",
                    "module": "B6",
                    "scenario": "S1"
                },
                {
                    "value": "0,00E+00",
                    "module": "B6",
                    "scenario": "S2"
                },
                {
                    "value": "0,00E+00",
                    "module": "C1",
                    "scenario": null
                },
                {
                    "value": "0,00E+00",
                    "module": "C2",
                    "scenario": null
                },
                {
                    "value": "6,72E-01",
                    "module": "C3",
                    "scenario": null
                },
                {
                    "value": "0,00E+00",
                    "module": "C4",
                    "scenario": null
                },
                {
                    "value": "0,00E+00",
                    "module": "D",
                    "scenario": null
                }
            ]
        },
        {
            "parameter": "MER",
            "values": [
                {
                    "value": "0,00E+00",
                    "module": "A1-A3",
                    "scenario": null
                },
                {
                    "value": "0,00E+00",
                    "module": "A4",
                    "scenario": null
                },
                {
                    "value": "0,00E+00",
                    "module": "A5",
                    "scenario": null
                },
                {
                    "value": "0,00E+00",
                    "module": "B6",
                    "scenario": "S1"
                },
                {
                    "value": "0,00E+00",
                    "module": "B6",
                    "scenario": "S2"
                },
                {
                    "value": "0,00E+00",
                    "module": "C1",
                    "scenario": null
                },
                {
                    "value": "0,00E+00",
                    "module": "C2",
                    "scenario": null
                },
                {
                    "value": "0,00E+00",
                    "module": "C3",
                    "scenario": null
                },
                {
                    "value": "0,00E+00",
                    "module": "C4",
                    "scenario": null
                },
                {
                    "value": "0,00E+00",
                    "module": "D",
                    "scenario": null
                }
            ]
        },
        {
            "parameter": "EEE",
            "values": [
                {
                    "value": "0,00E+00",
                    "module": "A1-A3",
                    "scenario": null
                },
                {
                    "value": "0,00E+00",
                    "module": "A4",
                    "scenario": null
                },
                {
                    "value": "0,00E+00",
                    "module": "A5",
                    "scenario": null
                },
                {
                    "value": "0,00E+00",
                    "module": "B6",
                    "scenario": "S1"
                },
                {
                    "value": "0,00E+00",
                    "module": "B6",
                    "scenario": "S2"
                },
                {
                    "value": "0,00E+00",
                    "module": "C1",
                    "scenario": null
                },
                {
                    "value": "0,00E+00",
                    "module": "C2",
                    "scenario": null
                },
                {
                    "value": "0,00E+00",
                    "module": "C3",
                    "scenario": null
                },
                {
                    "value": "0,00E+00",
                    "module": "C4",
                    "scenario": null
                },
                {
                    "value": "0,00E+00",
                    "module": "D",
                    "scenario": null
                }
            ]
        },
        {
            "parameter": "EET",
            "values": [
                {
                    "value": "0,00E+00",
                    "module": "A1-A3",
                    "scenario": null
                },
                {
                    "value": "0,00E+00",
                    "module": "A4",
                    "scenario": null
                },
                {
                    "value": "0,00E+00",
                    "module": "A5",
                    "scenario": null
                },
                {
                    "value": "0,00E+00",
                    "module": "B6",
                    "scenario": "S1"
                },
                {
                    "value": "0,00E+00",
                    "module": "B6",
                    "scenario": "S2"
                },
                {
                    "value": "0,00E+00",
                    "module": "C1",
                    "scenario": null
                },
                {
                    "value": "0,00E+00",
                    "module": "C2",
                    "scenario": null
                },
                {
                    "value": "0,00E+00",
                    "module": "C3",
                    "scenario": null
                },
                {
                    "value": "0,00E+00",
                    "module": "C4",
                    "scenario": null
                },
                {
                    "value": "0,00E+00",
                    "module": "D",
                    "scenario": null
                }
            ]
        }
    ]
}