{
    "product_name": "Component EPD Ringebu: Injection moulded PP fittings and gullies from Surnadal - used as material component in various finished mixed products",
    "epd_id": "NEPD-7772-7150",
    "compliance": [
        "EN 15804+A2",
        "ISO 14025",
        "ISO 21930"
    ],
    "producer_name": "Pipelife Norge AS",
    "environmental_impact": [
        {
            "parameter": "GWP-total",
            "values": [
                {
                    "value": "2,84E+00",
                    "module": "A1-A3",
                    "scenario": null
                },
                {
                    "value": "1,63E-02",
                    "module": "A4",
                    "scenario": null
                },
                {
                    "value": "0,00E+00",
                    "module": "A5",
                    "scenario": null
                },
                {
                    "value": "0,00E+00",
                    "module": "C1",
                    "scenario": null
                },
                {
                    "value": "0,00E+00",
                    "module": "C2",
                    "scenario": null
                },
                {
                    "value": "1,27E+00",
                    "module": "C3",
                    "scenario": null
                },
                {
                    "value": "5,79E-02",
                    "module": "C4",
                    "scenario": null
                },
                {
                    "value": "-7,40E-02",
                    "module": "D",
                    "scenario": null
                }
            ]
        },
        {
            "parameter": "GWP-fossil",
            "values": [
                {
                    "value": "2,82E+00",
                    "module": "A1-A3",
                    "scenario": null
                },
                {
                    "value": "1,63E-02",
                    "module": "A4",
                    "scenario": null
                },
                {
                    "value": "0,00E+00",
                    "module": "A5",
                    "scenario": null
                },
                {
                    "value": "0,00E+00",
                    "module": "C1",
                    "scenario": null
                },
                {
                    "value": "0,00E+00",
                    "module": "C2",
                    "scenario": null
                },
                {
                    "value": "1,27E+00",
                    "module": "C3",
                    "scenario": null
                },
                {
                    "value": "5,79E-02",
                    "module": "C4",
                    "scenario": null
                },
                {
                    "value": "-7,14E-02",
                    "module": "D",
                    "scenario": null
                }
            ]
        },
        {
            "parameter": "GWP-biogenic",
            "values": [
                {
                    "value": "2,17E-02",
                    "module": "A1-A3",
                    "scenario": null
                },
                {
                    "value": "6,76E-06",
                    "module": "A4",
                    "scenario": null
                },
                {
                    "value": "0,00E+00",
                    "module": "A5",
                    "scenario": null
                },
                {
                    "value": "0,00E+00",
                    "module": "C1",
                    "scenario": null
                },
                {
                    "value": "0,00E+00",
                    "module": "C2",
                    "scenario": null
                },
                {
                    "value": "1,05E-05",
                    "module": "C3",
                    "scenario": null
                },
                {
                    "value": "5,52E-06",
                    "module": "C4",
                    "scenario": null
                },
                {
                    "value": "-1,47E-04",
                    "module": "D",
                    "scenario": null
                }
            ]
        },
        {
            "parameter": "GWP-luluc",
            "values": [
                {
                    "value": "4,83E-03",
                    "module": "A1-A3",
                    "scenario": null
                },
                {
                    "value": "5,81E-06",
                    "module": "A4",
                    "scenario": null
                },
                {
                    "value": "0,00E+00",
                    "module": "A5",
                    "scenario": null
                },
                {
                    "value": "0,00E+00",
                    "module": "C1",
                    "scenario": null
                },
                {
                    "value": "0,00E+00",
                    "module": "C2",
                    "scenario": null
                },
                {
                    "value": "1,61E-06",
                    "module": "C3",
                    "scenario": null
                },
                {
                    "value": "1,24E-06",
                    "module": "C4",
                    "scenario": null
                },
                {
                    "value": "-2,46E-03",
                    "module": "D",
                    "scenario": null
                }
            ]
        },
        {
            "parameter": "ODP",
            "values": [
                {
                    "value": "1,95E-07",
                    "module": "A1-A3",
                    "scenario": null
                },
                {
                    "value": "3,70E-09",
                    "module": "A4",
                    "scenario": null
                },
                {
                    "value": "0,00E+00",
                    "module": "A5",
                    "scenario": null
                },
                {
                    "value": "0,00E+00",
                    "module": "C1",
                    "scenario": null
                },
                {
                    "value": "0,00E+00",
                    "module": "C2",
                    "scenario": null
                },
                {
                    "value": "1,00E-09",
                    "module": "C3",
                    "scenario": null
                },
                {
                    "value": "1,65E-09",
                    "module": "C4",
                    "scenario": null
                },
                {
                    "value": "-5,20E-03",
                    "module": "D",
                    "scenario": null
                }
            ]
        },
        {
            "parameter": "AP",
            "values": [
                {
                    "value": "1,29E-02",
                    "module": "A1-A3",
                    "scenario": null
                },
                {
                    "value": "4,69E-05",
                    "module": "A4",
                    "scenario": null
                },
                {
                    "value": "0,00E+00",
                    "module": "A5",
                    "scenario": null
                },
                {
                    "value": "0,00E+00",
                    "module": "C1",
                    "scenario": null
                },
                {
                    "value": "0,00E+00",
                    "module": "C2",
                    "scenario": null
                },
                {
                    "value": "1,61E-04",
                    "module": "C3",
                    "scenario": null
                },
                {
                    "value": "4,16E-05",
                    "module": "C4",
                    "scenario": null
                },
                {
                    "value": "-5,88E-04",
                    "module": "D",
                    "scenario": null
                }
            ]
        },
        {
            "parameter": "POCP",
            "values": [
                {
                    "value": "1,10E-02",
                    "module": "A1-A3",
                    "scenario": null
                },
                {
                    "value": "3,98E-05",
                    "module": "A4",
                    "scenario": null
                },
                {
                    "value": "0,00E+00",
                    "module": "A5",
                    "scenario": null
                },
                {
                    "value": "0,00E+00",
                    "module": "C1",
                    "scenario": null
                },
                {
                    "value": "0,00E+00",
                    "module": "C2",
                    "scenario": null
                },
                {
                    "value": "2,00E-04",
                    "module": "C3",
                    "scenario": null
                },
                {
                    "value": "5,88E-05",
                    "module": "C4",
                    "scenario": null
                },
                {
                    "value": "-5,73E-04",
                    "module": "D",
                    "scenario": null
                }
            ]
        },
        {
            "parameter": "ADPE",
            "values": [
                {
                    "value": "1,20E-04",
                    "module": "A1-A3",
                    "scenario": null
                },
                {
                    "value": "4,51E-07",
                    "module": "A4",
                    "scenario": null
                },
                {
                    "value": "0,00E+00",
                    "module": "A5",
                    "scenario": null
                },
                {
                    "value": "0,00E+00",
                    "module": "C1",
                    "scenario": null
                },
                {
                    "value": "0,00E+00",
                    "module": "C2",
                    "scenario": null
                },
                {
                    "value": "4,67E-08",
                    "module": "C3",
                    "scenario": null
                },
                {
                    "value": "4,23E-08",
                    "module": "C4",
                    "scenario": null
                },
                {
                    "value": "-7,10E-07",
                    "module": "D",
                    "scenario": null
                }
            ]
        },
        {
            "parameter": "ADPF",
            "values": [
                {
                    "value": "8,43E+01",
                    "module": "A1-A3",
                    "scenario": null
                },
                {
                    "value": "2,47E-01",
                    "module": "A4",
                    "scenario": null
                },
                {
                    "value": "0,00E+00",
                    "module": "A5",
                    "scenario": null
                },
                {
                    "value": "0,00E+00",
                    "module": "C1",
                    "scenario": null
                },
                {
                    "value": "0,00E+00",
                    "module": "C2",
                    "scenario": null
                },
                {
                    "value": "8,63E-02",
                    "module": "C3",
                    "scenario": null
                },
                {
                    "value": "1,22E-01",
                    "module": "C4",
                    "scenario": null
                },
                {
                    "value": "-1,02E+00",
                    "module": "D",
                    "scenario": null
                }
            ]
        },
        {
            "parameter": "WDP",
            "values": [
                {
                    "value": "6,47E+02",
                    "module": "A1-A3",
                    "scenario": null
                },
                {
                    "value": "2,39E-01",
                    "module": "A4",
                    "scenario": null
                },
                {
                    "value": "0,00E+00",
                    "module": "A5",
                    "scenario": null
                },
                {
                    "value": "0,00E+00",
                    "module": "C1",
                    "scenario": null
                },
                {
                    "value": "0,00E+00",
                    "module": "C2",
                    "scenario": null
                },
                {
                    "value": "2,01E-01",
                    "module": "C3",
                    "scenario": null
                },
                {
                    "value": "1,05E+00",
                    "module": "C4",
                    "scenario": null
                },
                {
                    "value": "-1,27E+01",
                    "module": "D",
                    "scenario": null
                }
            ]
        },
        {
            "parameter": "EP-freshwater",
            "values": [
                {
                    "value": "8,32E-05",
                    "module": "A1-A3",
                    "scenario": null
                },
                {
                    "value": "1,31E-07",
                    "module": "A4",
                    "scenario": null
                },
                {
                    "value": "0,00E+00",
                    "module": "A5",
                    "scenario": null
                },
                {
                    "value": "0,00E+00",
                    "module": "C1",
                    "scenario": null
                },
                {
                    "value": "0,00E+00",
                    "module": "C2",
                    "scenario": null
                },
                {
                    "value": "1,07E-07",
                    "module": "C3",
                    "scenario": null
                },
                {
                    "value": "6,24E-08",
                    "module": "C4",
                    "scenario": null
                },
                {
                    "value": "-6,34E-06",
                    "module": "D",
                    "scenario": null
                }
            ]
        },
        {
            "parameter": "EP-marine",
            "values": [
                {
                    "value": "2,56E-03",
                    "module": "A1-A3",
                    "scenario": null
                },
                {
                    "value": "9,29E-06",
                    "module": "A4",
                    "scenario": null
                },
                {
                    "value": "0,00E+00",
                    "module": "A5",
                    "scenario": null
                },
                {
                    "value": "0,00E+00",
                    "module": "C1",
                    "scenario": null
                },
                {
                    "value": "0,00E+00",
                    "module": "C2",
                    "scenario": null
                },
                {
                    "value": "7,68E-05",
                    "module": "C3",
                    "scenario": null
                },
                {
                    "value": "7,41E-05",
                    "module": "C4",
                    "scenario": null
                },
                {
                    "value": "-1,92E-04",
                    "module": "D",
                    "scenario": null
                }
            ]
        },
        {
            "parameter": "EP-terrestrial",
            "values": [
                {
                    "value": "2,83E-02",
                    "module": "A1-A3",
                    "scenario": null
                },
                {
                    "value": "1,04E-04",
                    "module": "A4",
                    "scenario": null
                },
                {
                    "value": "0,00E+00",
                    "module": "A5",
                    "scenario": null
                },
                {
                    "value": "0,00E+00",
                    "module": "C1",
                    "scenario": null
                },
                {
                    "value": "0,00E+00",
                    "module": "C2",
                    "scenario": null
                },
                {
                    "value": "8,31E-04",
                    "module": "C3",
                    "scenario": null
                },
                {
                    "value": "1,64E-04",
                    "module": "C4",
                    "scenario": null
                },
                {
                    "value": "-2,08E-03",
                    "module": "D",
                    "scenario": null
                }
            ]
        },
        {
            "parameter": "GWP-IOBC",
            "values": [
                {
                    "value": "2,74E+00",
                    "module": "A1-A3",
                    "scenario": null
                },
                {
                    "value": "1,63E-02",
                    "module": "A4",
                    "scenario": null
                },
                {
                    "value": "0,00E+00",
                    "module": "A5",
                    "scenario": null
                },
                {
                    "value": "0,00E+00",
                    "module": "C1",
                    "scenario": null
                },
                {
                    "value": "0,00E+00",
                    "module": "C2",
                    "scenario": null
                },
                {
                    "value": "1,27E+00",
                    "module": "C3",
                    "scenario": null
                },
                {
                    "value": "5,80E-02",
                    "module": "C4",
                    "scenario": null
                },
                {
                    "value": "-7,29E-02",
                    "module": "D",
                    "scenario": null
                }
            ]
        }
    ],
    "additional_environmental_impact": [
        {
            "parameter": "PM",
            "values": [
                {
                    "value": "1,40E-07",
                    "module": "A1-A3",
                    "scenario": null
                },
                {
                    "value": "1,00E-09",
                    "module": "A4",
                    "scenario": null
                },
                {
                    "value": "0,00E+00",
                    "module": "A5",
                    "scenario": null
                },
                {
                    "value": "0,00E+00",
                    "module": "C1",
                    "scenario": null
                },
                {
                    "value": "0,00E+00",
                    "module": "C2",
                    "scenario": null
                },
                {
                    "value": "7,52E-10",
                    "module": "C3",
                    "scenario": null
                },
                {
                    "value": "8,18E-10",
                    "module": "C4",
                    "scenario": null
                },
                {
                    "value": "-3,56E-08",
                    "module": "D",
                    "scenario": null
                }
            ]
        },
        {
            "parameter": "ETP-fw",
            "values": [
                {
                    "value": "5,31E+01",
                    "module": "A1-A3",
                    "scenario": null
                },
                {
                    "value": "1,83E-01",
                    "module": "A4",
                    "scenario": null
                },
                {
                    "value": "0,00E+00",
                    "module": "A5",
                    "scenario": null
                },
                {
                    "value": "0,00E+00",
                    "module": "C1",
                    "scenario": null
                },
                {
                    "value": "0,00E+00",
                    "module": "C2",
                    "scenario": null
                },
                {
                    "value": "2,55E-01",
                    "module": "C3",
                    "scenario": null
                },
                {
                    "value": "1,52E-01",
                    "module": "C4",
                    "scenario": null
                },
                {
                    "value": "-5,55E+00",
                    "module": "D",
                    "scenario": null
                }
            ]
        },
        {
            "parameter": "HTP-c",
            "values": [
                {
                    "value": "1,42E-09",
                    "module": "A1-A3",
                    "scenario": null
                },
                {
                    "value": "0,00E+00",
                    "module": "A4",
                    "scenario": null
                },
                {
                    "value": "0,00E+00",
                    "module": "A5",
                    "scenario": null
                },
                {
                    "value": "0,00E+00",
                    "module": "C1",
                    "scenario": null
                },
                {
                    "value": "0,00E+00",
                    "module": "C2",
                    "scenario": null
                },
                {
                    "value": "3,00E-11",
                    "module": "C3",
                    "scenario": null
                },
                {
                    "value": "4,00E-12",
                    "module": "C4",
                    "scenario": null
                },
                {
                    "value": "-1,01E-10",
                    "module": "D",
                    "scenario": null
                }
            ]
        },
        {
            "parameter": "HTP-nc",
            "values": [
                {
                    "value": "3,68E-08",
                    "module": "A1-A3",
                    "scenario": null
                },
                {
                    "value": "2,00E-10",
                    "module": "A4",
                    "scenario": null
                },
                {
                    "value": "0,00E+00",
                    "module": "A5",
                    "scenario": null
                },
                {
                    "value": "0,00E+00",
                    "module": "C1",
                    "scenario": null
                },
                {
                    "value": "0,00E+00",
                    "module": "C2",
                    "scenario": null
                },
                {
                    "value": "1,09E-09",
                    "module": "C3",
                    "scenario": null
                },
                {
                    "value": "1,14E-10",
                    "module": "C4",
                    "scenario": null
                },
                {
                    "value": "-5,32E-09",
                    "module": "D",
                    "scenario": null
                }
            ]
        },
        {
            "parameter": "SQP",
            "values": [
                {
                    "value": "4,64E+01",
                    "module": "A1-A3",
                    "scenario": null
                },
                {
                    "value": "1,73E-01",
                    "module": "A4",
                    "scenario": null
                },
                {
                    "value": "0,00E+00",
                    "module": "A5",
                    "scenario": null
                },
                {
                    "value": "0,00E+00",
                    "module": "C1",
                    "scenario": null
                },
                {
                    "value": "0,00E+00",
                    "module": "C2",
                    "scenario": null
                },
                {
                    "value": "1,09E-02",
                    "module": "C3",
                    "scenario": null
                },
                {
                    "value": "4,55E-01",
                    "module": "C4",
                    "scenario": null
                },
                {
                    "value": "-6,83E+00",
                    "module": "D",
                    "scenario": null
                }
            ]
        },
        {
            "parameter": "IRP",
            "values": [
                {
                    "value": "1,48E-01",
                    "module": "A1-A3",
                    "scenario": null
                },
                {
                    "value": "1,08E-03",
                    "module": "A4",
                    "scenario": null
                },
                {
                    "value": "0,00E+00",
                    "module": "A5",
                    "scenario": null
                },
                {
                    "value": "0,00E+00",
                    "module": "C1",
                    "scenario": null
                },
                {
                    "value": "0,00E+00",
                    "module": "C2",
                    "scenario": null
                },
                {
                    "value": "1,50E-04",
                    "module": "C3",
                    "scenario": null
                },
                {
                    "value": "5,90E-04",
                    "module": "C4",
                    "scenario": null
                },
                {
                    "value": "-6,52E-03",
                    "module": "D",
                    "scenario": null
                }
            ]
        }
    ],
    "resource_use": [
        {
            "parameter": "PERE",
            "values": [
                {
                    "value": "5,01E+01",
                    "module": "A1-A3",
                    "scenario": null
                },
                {
                    "value": "3,54E-03",
                    "module": "A4",
                    "scenario": null
                },
                {
                    "value": "0,00E+00",
                    "module": "A5",
                    "scenario": null
                },
                {
                    "value": "0,00E+00",
                    "module": "C1",
                    "scenario": null
                },
                {
                    "value": "0,00E+00",
                    "module": "C2",
                    "scenario": null
                },
                {
                    "value": "2,62E-03",
                    "module": "C3",
                    "scenario": null
                },
                {
                    "value": "5,75E-03",
                    "module": "C4",
                    "scenario": null
                },
                {
                    "value": "-6,31E+00",
                    "module": "D",
                    "scenario": null
                }
            ]
        },
        {
            "parameter": "PERM",
            "values": [
                {
                    "value": "0,00E+00",
                    "module": "A1-A3",
                    "scenario": null
                },
                {
                    "value": "0,00E+00",
                    "module": "A4",
                    "scenario": null
                },
                {
                    "value": "0,00E+00",
                    "module": "A5",
                    "scenario": null
                },
                {
                    "value": "0,00E+00",
                    "module": "C1",
                    "scenario": null
                },
                {
                    "value": "0,00E+00",
                    "module": "C2",
                    "scenario": null
                },
                {
                    "value": "0,00E+00",
                    "module": "C3",
                    "scenario": null
                },
                {
                    "value": "0,00E+00",
                    "module": "C4",
                    "scenario": null
                },
                {
                    "value": "0,00E+00",
                    "module": "D",
                    "scenario": null
                }
            ]
        },
        {
            "parameter": "PERT",
            "values": [
                {
                    "value": "5,01E+01",
                    "module": "A1-A3",
                    "scenario": null
                },
                {
                    "value": "3,54E-03",
                    "module": "A4",
                    "scenario": null
                },
                {
                    "value": "0,00E+00",
                    "module": "A5",
                    "scenario": null
                },
                {
                    "value": "0,00E+00",
                    "module": "C1",
                    "scenario": null
                },
                {
                    "value": "0,00E+00",
                    "module": "C2",
                    "scenario": null
                },
                {
                    "value": "2,62E-03",
                    "module": "C3",
                    "scenario": null
                },
                {
                    "value": "5,75E-03",
                    "module": "C4",
                    "scenario": null
                },
                {
                    "value": "-6,31E+00",
                    "module": "D",
                    "scenario": null
                }
            ]
        },
        {
            "parameter": "PENRE",
            "values": [
                {
                    "value": "5,41E+01",
                    "module": "A1-A3",
                    "scenario": null
                },
                {
                    "value": "2,47E-01",
                    "module": "A4",
                    "scenario": null
                },
                {
                    "value": "0,00E+00",
                    "module": "A5",
                    "scenario": null
                },
                {
                    "value": "0,00E+00",
                    "module": "C1",
                    "scenario": null
                },
                {
                    "value": "0,00E+00",
                    "module": "C2",
                    "scenario": null
                },
                {
                    "value": "8,63E-02",
                    "module": "C3",
                    "scenario": null
                },
                {
                    "value": "1,22E-01",
                    "module": "C4",
                    "scenario": null
                },
                {
                    "value": "-1,02E+00",
                    "module": "D",
                    "scenario": null
                }
            ]
        },
        {
            "parameter": "PENRM",
            "values": [
                {
                    "value": "3,26E+01",
                    "module": "A1-A3",
                    "scenario": null
                },
                {
                    "value": "0,00E+00",
                    "module": "A4",
                    "scenario": null
                },
                {
                    "value": "0,00E+00",
                    "module": "A5",
                    "scenario": null
                },
                {
                    "value": "0,00E+00",
                    "module": "C1",
                    "scenario": null
                },
                {
                    "value": "0,00E+00",
                    "module": "C2",
                    "scenario": null
                },
                {
                    "value": "-3,26E+01",
                    "module": "C3",
                    "scenario": null
                },
                {
                    "value": "0,00E+00",
                    "module": "C4",
                    "scenario": null
                },
                {
                    "value": "0,00E+00",
                    "module": "D",
                    "scenario": null
                }
            ]
        },
        {
            "parameter": "PENRT",
            "values": [
                {
                    "value": "8,67E+01",
                    "module": "A1-A3",
                    "scenario": null
                },
                {
                    "value": "2,47E-01",
                    "module": "A4",
                    "scenario": null
                },
                {
                    "value": "0,00E+00",
                    "module": "A5",
                    "scenario": null
                },
                {
                    "value": "0,00E+00",
                    "module": "C1",
                    "scenario": null
                },
                {
                    "value": "0,00E+00",
                    "module": "C2",
                    "scenario": null
                },
                {
                    "value": "-3,25E+01",
                    "module": "C3",
                    "scenario": null
                },
                {
                    "value": "1,22E-01",
                    "module": "C4",
                    "scenario": null
                },
                {
                    "value": "-1,02E+00",
                    "module": "D",
                    "scenario": null
                }
            ]
        },
        {
            "parameter": "SM",
            "values": [
                {
                    "value": "0,00E+00",
                    "module": "A1-A3",
                    "scenario": null
                },
                {
                    "value": "0,00E+00",
                    "module": "A4",
                    "scenario": null
                },
                {
                    "value": "0,00E+00",
                    "module": "A5",
                    "scenario": null
                },
                {
                    "value": "0,00E+00",
                    "module": "C1",
                    "scenario": null
                },
                {
                    "value": "0,00E+00",
                    "module": "C2",
                    "scenario": null
                },
                {
                    "value": "0,00E+00",
                    "module": "C3",
                    "scenario": null
                },
                {
                    "value": "0,00E+00",
                    "module": "C4",
                    "scenario": null
                },
                {
                    "value": "0,00E+00",
                    "module": "D",
                    "scenario": null
                }
            ]
        },
        {
            "parameter": "RSF",
            "values": [
                {
                    "value": "1,25E-01",
                    "module": "A1-A3",
                    "scenario": null
                },
                {
                    "value": "1,26E-04",
                    "module": "A4",
                    "scenario": null
                },
                {
                    "value": "0,00E+00",
                    "module": "A5",
                    "scenario": null
                },
                {
                    "value": "0,00E+00",
                    "module": "C1",
                    "scenario": null
                },
                {
                    "value": "0,00E+00",
                    "module": "C2",
                    "scenario": null
                },
                {
                    "value": "7,21E-05",
                    "module": "C3",
                    "scenario": null
                },
                {
                    "value": "1,21E-04",
                    "module": "C4",
                    "scenario": null
                },
                {
                    "value": "-1,10E-03",
                    "module": "D",
                    "scenario": null
                }
            ]
        },
        {
            "parameter": "NRSF",
            "values": [
                {
                    "value": "9,97E-02",
                    "module": "A1-A3",
                    "scenario": null
                },
                {
                    "value": "4,52E-04",
                    "module": "A4",
                    "scenario": null
                },
                {
                    "value": "0,00E+00",
                    "module": "A5",
                    "scenario": null
                },
                {
                    "value": "0,00E+00",
                    "module": "C1",
                    "scenario": null
                },
                {
                    "value": "0,00E+00",
                    "module": "C2",
                    "scenario": null
                },
                {
                    "value": "0,00E+00",
                    "module": "C3",
                    "scenario": null
                },
                {
                    "value": "1,97E-03",
                    "module": "C4",
                    "scenario": null
                },
                {
                    "value": "-3,74E-01",
                    "module": "D",
                    "scenario": null
                }
            ]
        },
        {
            "parameter": "FW",
            "values": [
                {
                    "value": "3,47E-01",
                    "module": "A1-A3",
                    "scenario": null
                },
                {
                    "value": "2,64E-05",
                    "module": "A4",
                    "scenario": null
                },
                {
                    "value": "0,00E+00",
                    "module": "A5",
                    "scenario": null
                },
                {
                    "value": "0,00E+00",
                    "module": "C1",
                    "scenario": null
                },
                {
                    "value": "0,00E+00",
                    "module": "C2",
                    "scenario": null
                },
                {
                    "value": "2,38E-04",
                    "module": "C3",
                    "scenario": null
                },
                {
                    "value": "1,50E-04",
                    "module": "C4",
                    "scenario": null
                },
                {
                    "value": "-7,59E-03",
                    "module": "D",
                    "scenario": null
                }
            ]
        }
    ],
    "end_of_life_waste": [
        {
            "parameter": "HWD",
            "values": [
                {
                    "value": "7,90E-03",
                    "module": "A1-A3",
                    "scenario": null
                },
                {
                    "value": "1,27E-05",
                    "module": "A4",
                    "scenario": null
                },
                {
                    "value": "0,00E+00",
                    "module": "A5",
                    "scenario": null
                },
                {
                    "value": "0,00E+00",
                    "module": "C1",
                    "scenario": null
                },
                {
                    "value": "0,00E+00",
                    "module": "C2",
                    "scenario": null
                },
                {
                    "value": "0,00E+00",
                    "module": "C3",
                    "scenario": null
                },
                {
                    "value": "1,26E-02",
                    "module": "C4",
                    "scenario": null
                },
                {
                    "value": "-4,80E-05",
                    "module": "D",
                    "scenario": null
                }
            ]
        },
        {
            "parameter": "NHWD",
            "values": [
                {
                    "value": "4,62E-01",
                    "module": "A1-A3",
                    "scenario": null
                },
                {
                    "value": "1,20E-02",
                    "module": "A4",
                    "scenario": null
                },
                {
                    "value": "0,00E+00",
                    "module": "A5",
                    "scenario": null
                },
                {
                    "value": "0,00E+00",
                    "module": "C1",
                    "scenario": null
                },
                {
                    "value": "0,00E+00",
                    "module": "C2",
                    "scenario": null
                },
                {
                    "value": "0,00E+00",
                    "module": "C3",
                    "scenario": null
                },
                {
                    "value": "5,07E-01",
                    "module": "C4",
                    "scenario": null
                },
                {
                    "value": "-2,41E-02",
                    "module": "D",
                    "scenario": null
                }
            ]
        },
        {
            "parameter": "RWD",
            "values": [
                {
                    "value": "1,29E-04",
                    "module": "A1-A3",
                    "scenario": null
                },
                {
                    "value": "1,68E-06",
                    "module": "A4",
                    "scenario": null
                },
                {
                    "value": "0,00E+00",
                    "module": "A5",
                    "scenario": null
                },
                {
                    "value": "0,00E+00",
                    "module": "C1",
                    "scenario": null
                },
                {
                    "value": "0,00E+00",
                    "module": "C2",
                    "scenario": null
                },
                {
                    "value": "0,00E+00",
                    "module": "C3",
                    "scenario": null
                },
                {
                    "value": "8,02E-07",
                    "module": "C4",
                    "scenario": null
                },
                {
                    "value": "-5,34E-06",
                    "module": "D",
                    "scenario": null
                }
            ]
        }
    ],
    "end_of_life_flow": [
        {
            "parameter": "CRU",
            "values": [
                {
                    "value": "0,00E+00",
                    "module": "A1-A3",
                    "scenario": null
                },
                {
                    "value": "0,00E+00",
                    "module": "A4",
                    "scenario": null
                },
                {
                    "value": "0,00E+00",
                    "module": "A5",
                    "scenario": null
                },
                {
                    "value": "0,00E+00",
                    "module": "C1",
                    "scenario": null
                },
                {
                    "value": "0,00E+00",
                    "module": "C2",
                    "scenario": null
                },
                {
                    "value": "0,00E+00",
                    "module": "C3",
                    "scenario": null
                },
                {
                    "value": "0,00E+00",
                    "module": "C4",
                    "scenario": null
                },
                {
                    "value": "0,00E+00",
                    "module": "D",
                    "scenario": null
                }
            ]
        },
        {
            "parameter": "MFR",
            "values": [
                {
                    "value": "0,00E+00",
                    "module": "A1-A3",
                    "scenario": null
                },
                {
                    "value": "0,00E+00",
                    "module": "A4",
                    "scenario": null
                },
                {
                    "value": "0,00E+00",
                    "module": "A5",
                    "scenario": null
                },
                {
                    "value": "0,00E+00",
                    "module": "C1",
                    "scenario": null
                },
                {
                    "value": "0,00E+00",
                    "module": "C2",
                    "scenario": null
                },
                {
                    "value": "0,00E+00",
                    "module": "C3",
                    "scenario": null
                },
                {
                    "value": "4,48E-05",
                    "module": "C4",
                    "scenario": null
                },
                {
                    "value": "0,00E+00",
                    "module": "D",
                    "scenario": null
                }
            ]
        },
        {
            "parameter": "MER",
            "values": [
                {
                    "value": "0,00E+00",
                    "module": "A1-A3",
                    "scenario": null
                },
                {
                    "value": "0,00E+00",
                    "module": "A4",
                    "scenario": null
                },
                {
                    "value": "0,00E+00",
                    "module": "A5",
                    "scenario": null
                },
                {
                    "value": "0,00E+00",
                    "module": "C1",
                    "scenario": null
                },
                {
                    "value": "0,00E+00",
                    "module": "C2",
                    "scenario": null
                },
                {
                    "value": "5,00E-01",
                    "module": "C3",
                    "scenario": null
                },
                {
                    "value": "1,10E-06",
                    "module": "C4",
                    "scenario": null
                },
                {
                    "value": "0,00E+00",
                    "module": "D",
                    "scenario": null
                }
            ]
        },
        {
            "parameter": "EEE",
            "values": [
                {
                    "value": "0,00E+00",
                    "module": "A1-A3",
                    "scenario": null
                },
                {
                    "value": "0,00E+00",
                    "module": "A4",
                    "scenario": null
                },
                {
                    "value": "0,00E+00",
                    "module": "A5",
                    "scenario": null
                },
                {
                    "value": "0,00E+00",
                    "module": "C1",
                    "scenario": null
                },
                {
                    "value": "0,00E+00",
                    "module": "C2",
                    "scenario": null
                },
                {
                    "value": "8,14E-01",
                    "module": "C3",
                    "scenario": null
                },
                {
                    "value": "7,12E-05",
                    "module": "C4",
                    "scenario": null
                },
                {
                    "value": "0,00E+00",
                    "module": "D",
                    "scenario": null
                }
            ]
        },
        {
            "parameter": "EET",
            "values": [
                {
                    "value": "0,00E+00",
                    "module": "A1-A3",
                    "scenario": null
                },
                {
                    "value": "0,00E+00",
                    "module": "A4",
                    "scenario": null
                },
                {
                    "value": "0,00E+00",
                    "module": "A5",
                    "scenario": null
                },
                {
                    "value": "0,00E+00",
                    "module": "C1",
                    "scenario": null
                },
                {
                    "value": "0,00E+00",
                    "module": "C2",
                    "scenario": null
                },
                {
                    "value": "1,23E+01",
                    "module": "C3",
                    "scenario": null
                },
                {
                    "value": "1,08E-03",
                    "module": "C4",
                    "scenario": null
                },
                {
                    "value": "0,00E+00",
                    "module": "D",
                    "scenario": null
                }
            ]
        }
    ]
}