{
    "product_name": "Component EPD Ringebu: Extruded PVC-U pipe systems from Surnadal - used as material component in various finished mixed products",
    "epd_id": "NEPD-7774-7145",
    "compliance": [
        "EN 15804+A2",
        "ISO 14025",
        "ISO 21930"
    ],
    "producer_name": "Pipelife Norge AS",
    "environmental_impact": [
        {
            "parameter": "GWP-total",
            "values": [
                {
                    "value": "2,13E+00",
                    "module": "A1-A3",
                    "scenario": null
                },
                {
                    "value": "1,63E-02",
                    "module": "A4",
                    "scenario": null
                },
                {
                    "value": "0,00E+00",
                    "module": "A5",
                    "scenario": null
                },
                {
                    "value": "0,00E+00",
                    "module": "C1",
                    "scenario": null
                },
                {
                    "value": "0,00E+00",
                    "module": "C2",
                    "scenario": null
                },
                {
                    "value": "1,00E+00",
                    "module": "C3",
                    "scenario": null
                },
                {
                    "value": "7,60E-02",
                    "module": "C4",
                    "scenario": null
                },
                {
                    "value": "-4,65E-02",
                    "module": "D",
                    "scenario": null
                }
            ]
        },
        {
            "parameter": "GWP-fossil",
            "values": [
                {
                    "value": "2,12E+00",
                    "module": "A1-A3",
                    "scenario": null
                },
                {
                    "value": "1,63E-02",
                    "module": "A4",
                    "scenario": null
                },
                {
                    "value": "0,00E+00",
                    "module": "A5",
                    "scenario": null
                },
                {
                    "value": "0,00E+00",
                    "module": "C1",
                    "scenario": null
                },
                {
                    "value": "0,00E+00",
                    "module": "C2",
                    "scenario": null
                },
                {
                    "value": "1,00E+00",
                    "module": "C3",
                    "scenario": null
                },
                {
                    "value": "7,60E-02",
                    "module": "C4",
                    "scenario": null
                },
                {
                    "value": "-4,49E-02",
                    "module": "D",
                    "scenario": null
                }
            ]
        },
        {
            "parameter": "GWP-biogenic",
            "values": [
                {
                    "value": "7,18E-03",
                    "module": "A1-A3",
                    "scenario": null
                },
                {
                    "value": "6,76E-06",
                    "module": "A4",
                    "scenario": null
                },
                {
                    "value": "0,00E+00",
                    "module": "A5",
                    "scenario": null
                },
                {
                    "value": "0,00E+00",
                    "module": "C1",
                    "scenario": null
                },
                {
                    "value": "0,00E+00",
                    "module": "C2",
                    "scenario": null
                },
                {
                    "value": "4,08E-04",
                    "module": "C3",
                    "scenario": null
                },
                {
                    "value": "1,42E-05",
                    "module": "C4",
                    "scenario": null
                },
                {
                    "value": "-9,26E-05",
                    "module": "D",
                    "scenario": null
                }
            ]
        },
        {
            "parameter": "GWP-luluc",
            "values": [
                {
                    "value": "1,74E-03",
                    "module": "A1-A3",
                    "scenario": null
                },
                {
                    "value": "5,81E-06",
                    "module": "A4",
                    "scenario": null
                },
                {
                    "value": "0,00E+00",
                    "module": "A5",
                    "scenario": null
                },
                {
                    "value": "0,00E+00",
                    "module": "C1",
                    "scenario": null
                },
                {
                    "value": "0,00E+00",
                    "module": "C2",
                    "scenario": null
                },
                {
                    "value": "7,83E-05",
                    "module": "C3",
                    "scenario": null
                },
                {
                    "value": "3,42E-06",
                    "module": "C4",
                    "scenario": null
                },
                {
                    "value": "-1,55E-03",
                    "module": "D",
                    "scenario": null
                }
            ]
        },
        {
            "parameter": "ODP",
            "values": [
                {
                    "value": "1,12E-06",
                    "module": "A1-A3",
                    "scenario": null
                },
                {
                    "value": "3,70E-09",
                    "module": "A4",
                    "scenario": null
                },
                {
                    "value": "0,00E+00",
                    "module": "A5",
                    "scenario": null
                },
                {
                    "value": "0,00E+00",
                    "module": "C1",
                    "scenario": null
                },
                {
                    "value": "0,00E+00",
                    "module": "C2",
                    "scenario": null
                },
                {
                    "value": "3,29E-08",
                    "module": "C3",
                    "scenario": null
                },
                {
                    "value": "2,78E-09",
                    "module": "C4",
                    "scenario": null
                },
                {
                    "value": "-3,27E-03",
                    "module": "D",
                    "scenario": null
                }
            ]
        },
        {
            "parameter": "AP",
            "values": [
                {
                    "value": "9,81E-03",
                    "module": "A1-A3",
                    "scenario": null
                },
                {
                    "value": "4,69E-05",
                    "module": "A4",
                    "scenario": null
                },
                {
                    "value": "0,00E+00",
                    "module": "A5",
                    "scenario": null
                },
                {
                    "value": "0,00E+00",
                    "module": "C1",
                    "scenario": null
                },
                {
                    "value": "0,00E+00",
                    "module": "C2",
                    "scenario": null
                },
                {
                    "value": "5,79E-04",
                    "module": "C3",
                    "scenario": null
                },
                {
                    "value": "9,10E-05",
                    "module": "C4",
                    "scenario": null
                },
                {
                    "value": "-3,70E-04",
                    "module": "D",
                    "scenario": null
                }
            ]
        },
        {
            "parameter": "POCP",
            "values": [
                {
                    "value": "6,85E-03",
                    "module": "A1-A3",
                    "scenario": null
                },
                {
                    "value": "3,98E-05",
                    "module": "A4",
                    "scenario": null
                },
                {
                    "value": "0,00E+00",
                    "module": "A5",
                    "scenario": null
                },
                {
                    "value": "0,00E+00",
                    "module": "C1",
                    "scenario": null
                },
                {
                    "value": "0,00E+00",
                    "module": "C2",
                    "scenario": null
                },
                {
                    "value": "4,29E-04",
                    "module": "C3",
                    "scenario": null
                },
                {
                    "value": "1,03E-04",
                    "module": "C4",
                    "scenario": null
                },
                {
                    "value": "-3,60E-04",
                    "module": "D",
                    "scenario": null
                }
            ]
        },
        {
            "parameter": "ADPE",
            "values": [
                {
                    "value": "5,18E-05",
                    "module": "A1-A3",
                    "scenario": null
                },
                {
                    "value": "4,51E-07",
                    "module": "A4",
                    "scenario": null
                },
                {
                    "value": "0,00E+00",
                    "module": "A5",
                    "scenario": null
                },
                {
                    "value": "0,00E+00",
                    "module": "C1",
                    "scenario": null
                },
                {
                    "value": "0,00E+00",
                    "module": "C2",
                    "scenario": null
                },
                {
                    "value": "2,11E-06",
                    "module": "C3",
                    "scenario": null
                },
                {
                    "value": "9,72E-08",
                    "module": "C4",
                    "scenario": null
                },
                {
                    "value": "-4,46E-07",
                    "module": "D",
                    "scenario": null
                }
            ]
        },
        {
            "parameter": "ADPF",
            "values": [
                {
                    "value": "5,24E+01",
                    "module": "A1-A3",
                    "scenario": null
                },
                {
                    "value": "2,47E-01",
                    "module": "A4",
                    "scenario": null
                },
                {
                    "value": "0,00E+00",
                    "module": "A5",
                    "scenario": null
                },
                {
                    "value": "0,00E+00",
                    "module": "C1",
                    "scenario": null
                },
                {
                    "value": "0,00E+00",
                    "module": "C2",
                    "scenario": null
                },
                {
                    "value": "1,32E+00",
                    "module": "C3",
                    "scenario": null
                },
                {
                    "value": "2,31E-01",
                    "module": "C4",
                    "scenario": null
                },
                {
                    "value": "-6,42E-01",
                    "module": "D",
                    "scenario": null
                }
            ]
        },
        {
            "parameter": "WDP",
            "values": [
                {
                    "value": "1,67E+02",
                    "module": "A1-A3",
                    "scenario": null
                },
                {
                    "value": "2,39E-01",
                    "module": "A4",
                    "scenario": null
                },
                {
                    "value": "0,00E+00",
                    "module": "A5",
                    "scenario": null
                },
                {
                    "value": "0,00E+00",
                    "module": "C1",
                    "scenario": null
                },
                {
                    "value": "0,00E+00",
                    "module": "C2",
                    "scenario": null
                },
                {
                    "value": "2,69E+01",
                    "module": "C3",
                    "scenario": null
                },
                {
                    "value": "2,95E+00",
                    "module": "C4",
                    "scenario": null
                },
                {
                    "value": "-7,99E+00",
                    "module": "D",
                    "scenario": null
                }
            ]
        },
        {
            "parameter": "EP-freshwater",
            "values": [
                {
                    "value": "8,78E-05",
                    "module": "A1-A3",
                    "scenario": null
                },
                {
                    "value": "1,31E-07",
                    "module": "A4",
                    "scenario": null
                },
                {
                    "value": "0,00E+00",
                    "module": "A5",
                    "scenario": null
                },
                {
                    "value": "0,00E+00",
                    "module": "C1",
                    "scenario": null
                },
                {
                    "value": "0,00E+00",
                    "module": "C2",
                    "scenario": null
                },
                {
                    "value": "2,95E-06",
                    "module": "C3",
                    "scenario": null
                },
                {
                    "value": "3,21E-07",
                    "module": "C4",
                    "scenario": null
                },
                {
                    "value": "-3,99E-06",
                    "module": "D",
                    "scenario": null
                }
            ]
        },
        {
            "parameter": "EP-marine",
            "values": [
                {
                    "value": "1,87E-03",
                    "module": "A1-A3",
                    "scenario": null
                },
                {
                    "value": "9,29E-06",
                    "module": "A4",
                    "scenario": null
                },
                {
                    "value": "0,00E+00",
                    "module": "A5",
                    "scenario": null
                },
                {
                    "value": "0,00E+00",
                    "module": "C1",
                    "scenario": null
                },
                {
                    "value": "0,00E+00",
                    "module": "C2",
                    "scenario": null
                },
                {
                    "value": "1,41E-04",
                    "module": "C3",
                    "scenario": null
                },
                {
                    "value": "8,83E-05",
                    "module": "C4",
                    "scenario": null
                },
                {
                    "value": "-1,21E-04",
                    "module": "D",
                    "scenario": null
                }
            ]
        },
        {
            "parameter": "EP-terrestrial",
            "values": [
                {
                    "value": "2,02E-02",
                    "module": "A1-A3",
                    "scenario": null
                },
                {
                    "value": "1,04E-04",
                    "module": "A4",
                    "scenario": null
                },
                {
                    "value": "0,00E+00",
                    "module": "A5",
                    "scenario": null
                },
                {
                    "value": "0,00E+00",
                    "module": "C1",
                    "scenario": null
                },
                {
                    "value": "0,00E+00",
                    "module": "C2",
                    "scenario": null
                },
                {
                    "value": "1,52E-03",
                    "module": "C3",
                    "scenario": null
                },
                {
                    "value": "3,29E-04",
                    "module": "C4",
                    "scenario": null
                },
                {
                    "value": "-1,31E-03",
                    "module": "D",
                    "scenario": null
                }
            ]
        },
        {
            "parameter": "GWP-IOBC",
            "values": [
                {
                    "value": "2,13E+00",
                    "module": "A1-A3",
                    "scenario": null
                },
                {
                    "value": "1,63E-02",
                    "module": "A4",
                    "scenario": null
                },
                {
                    "value": "0,00E+00",
                    "module": "A5",
                    "scenario": null
                },
                {
                    "value": "0,00E+00",
                    "module": "C1",
                    "scenario": null
                },
                {
                    "value": "0,00E+00",
                    "module": "C2",
                    "scenario": null
                },
                {
                    "value": "1,00E+00",
                    "module": "C3",
                    "scenario": null
                },
                {
                    "value": "7,69E-02",
                    "module": "C4",
                    "scenario": null
                },
                {
                    "value": "-4,58E-02",
                    "module": "D",
                    "scenario": null
                }
            ]
        }
    ],
    "additional_environmental_impact": [
        {
            "parameter": "PM",
            "values": [
                {
                    "value": "8,56E-08",
                    "module": "A1-A3",
                    "scenario": null
                },
                {
                    "value": "1,00E-09",
                    "module": "A4",
                    "scenario": null
                },
                {
                    "value": "0,00E+00",
                    "module": "A5",
                    "scenario": null
                },
                {
                    "value": "0,00E+00",
                    "module": "C1",
                    "scenario": null
                },
                {
                    "value": "0,00E+00",
                    "module": "C2",
                    "scenario": null
                },
                {
                    "value": "3,77E-09",
                    "module": "C3",
                    "scenario": null
                },
                {
                    "value": "1,27E-09",
                    "module": "C4",
                    "scenario": null
                },
                {
                    "value": "-2,24E-08",
                    "module": "D",
                    "scenario": null
                }
            ]
        },
        {
            "parameter": "ETP-fw",
            "values": [
                {
                    "value": "3,27E+01",
                    "module": "A1-A3",
                    "scenario": null
                },
                {
                    "value": "1,83E-01",
                    "module": "A4",
                    "scenario": null
                },
                {
                    "value": "0,00E+00",
                    "module": "A5",
                    "scenario": null
                },
                {
                    "value": "0,00E+00",
                    "module": "C1",
                    "scenario": null
                },
                {
                    "value": "0,00E+00",
                    "module": "C2",
                    "scenario": null
                },
                {
                    "value": "6,32E+01",
                    "module": "C3",
                    "scenario": null
                },
                {
                    "value": "4,67E-01",
                    "module": "C4",
                    "scenario": null
                },
                {
                    "value": "-3,49E+00",
                    "module": "D",
                    "scenario": null
                }
            ]
        },
        {
            "parameter": "HTP-c",
            "values": [
                {
                    "value": "1,31E-09",
                    "module": "A1-A3",
                    "scenario": null
                },
                {
                    "value": "0,00E+00",
                    "module": "A4",
                    "scenario": null
                },
                {
                    "value": "0,00E+00",
                    "module": "A5",
                    "scenario": null
                },
                {
                    "value": "0,00E+00",
                    "module": "C1",
                    "scenario": null
                },
                {
                    "value": "0,00E+00",
                    "module": "C2",
                    "scenario": null
                },
                {
                    "value": "1,41E-10",
                    "module": "C3",
                    "scenario": null
                },
                {
                    "value": "2,00E-11",
                    "module": "C4",
                    "scenario": null
                },
                {
                    "value": "-6,40E-11",
                    "module": "D",
                    "scenario": null
                }
            ]
        },
        {
            "parameter": "HTP-nc",
            "values": [
                {
                    "value": "3,72E-08",
                    "module": "A1-A3",
                    "scenario": null
                },
                {
                    "value": "2,00E-10",
                    "module": "A4",
                    "scenario": null
                },
                {
                    "value": "0,00E+00",
                    "module": "A5",
                    "scenario": null
                },
                {
                    "value": "0,00E+00",
                    "module": "C1",
                    "scenario": null
                },
                {
                    "value": "0,00E+00",
                    "module": "C2",
                    "scenario": null
                },
                {
                    "value": "1,49E-08",
                    "module": "C3",
                    "scenario": null
                },
                {
                    "value": "7,44E-10",
                    "module": "C4",
                    "scenario": null
                },
                {
                    "value": "-3,34E-09",
                    "module": "D",
                    "scenario": null
                }
            ]
        },
        {
            "parameter": "SQP",
            "values": [
                {
                    "value": "1,04E+01",
                    "module": "A1-A3",
                    "scenario": null
                },
                {
                    "value": "1,73E-01",
                    "module": "A4",
                    "scenario": null
                },
                {
                    "value": "0,00E+00",
                    "module": "A5",
                    "scenario": null
                },
                {
                    "value": "0,00E+00",
                    "module": "C1",
                    "scenario": null
                },
                {
                    "value": "0,00E+00",
                    "module": "C2",
                    "scenario": null
                },
                {
                    "value": "4,80E-01",
                    "module": "C3",
                    "scenario": null
                },
                {
                    "value": "8,14E-01",
                    "module": "C4",
                    "scenario": null
                },
                {
                    "value": "-4,29E+00",
                    "module": "D",
                    "scenario": null
                }
            ]
        },
        {
            "parameter": "IRP",
            "values": [
                {
                    "value": "1,18E-01",
                    "module": "A1-A3",
                    "scenario": null
                },
                {
                    "value": "1,08E-03",
                    "module": "A4",
                    "scenario": null
                },
                {
                    "value": "0,00E+00",
                    "module": "A5",
                    "scenario": null
                },
                {
                    "value": "0,00E+00",
                    "module": "C1",
                    "scenario": null
                },
                {
                    "value": "0,00E+00",
                    "module": "C2",
                    "scenario": null
                },
                {
                    "value": "6,40E-03",
                    "module": "C3",
                    "scenario": null
                },
                {
                    "value": "1,17E-03",
                    "module": "C4",
                    "scenario": null
                },
                {
                    "value": "-4,10E-03",
                    "module": "D",
                    "scenario": null
                }
            ]
        }
    ],
    "resource_use": [
        {
            "parameter": "PERE",
            "values": [
                {
                    "value": "3,22E+00",
                    "module": "A1-A3",
                    "scenario": null
                },
                {
                    "value": "3,54E-03",
                    "module": "A4",
                    "scenario": null
                },
                {
                    "value": "0,00E+00",
                    "module": "A5",
                    "scenario": null
                },
                {
                    "value": "0,00E+00",
                    "module": "C1",
                    "scenario": null
                },
                {
                    "value": "0,00E+00",
                    "module": "C2",
                    "scenario": null
                },
                {
                    "value": "1,68E-01",
                    "module": "C3",
                    "scenario": null
                },
                {
                    "value": "1,58E-02",
                    "module": "C4",
                    "scenario": null
                },
                {
                    "value": "-3,96E+00",
                    "module": "D",
                    "scenario": null
                }
            ]
        },
        {
            "parameter": "PERM",
            "values": [
                {
                    "value": "0,00E+00",
                    "module": "A1-A3",
                    "scenario": null
                },
                {
                    "value": "0,00E+00",
                    "module": "A4",
                    "scenario": null
                },
                {
                    "value": "0,00E+00",
                    "module": "A5",
                    "scenario": null
                },
                {
                    "value": "0,00E+00",
                    "module": "C1",
                    "scenario": null
                },
                {
                    "value": "0,00E+00",
                    "module": "C2",
                    "scenario": null
                },
                {
                    "value": "0,00E+00",
                    "module": "C3",
                    "scenario": null
                },
                {
                    "value": "0,00E+00",
                    "module": "C4",
                    "scenario": null
                },
                {
                    "value": "0,00E+00",
                    "module": "D",
                    "scenario": null
                }
            ]
        },
        {
            "parameter": "PERT",
            "values": [
                {
                    "value": "3,22E+00",
                    "module": "A1-A3",
                    "scenario": null
                },
                {
                    "value": "3,54E-03",
                    "module": "A4",
                    "scenario": null
                },
                {
                    "value": "0,00E+00",
                    "module": "A5",
                    "scenario": null
                },
                {
                    "value": "0,00E+00",
                    "module": "C1",
                    "scenario": null
                },
                {
                    "value": "0,00E+00",
                    "module": "C2",
                    "scenario": null
                },
                {
                    "value": "1,68E-01",
                    "module": "C3",
                    "scenario": null
                },
                {
                    "value": "1,58E-02",
                    "module": "C4",
                    "scenario": null
                },
                {
                    "value": "-3,96E+00",
                    "module": "D",
                    "scenario": null
                }
            ]
        },
        {
            "parameter": "PENRE",
            "values": [
                {
                    "value": "3,16E+01",
                    "module": "A1-A3",
                    "scenario": null
                },
                {
                    "value": "2,47E-01",
                    "module": "A4",
                    "scenario": null
                },
                {
                    "value": "0,00E+00",
                    "module": "A5",
                    "scenario": null
                },
                {
                    "value": "0,00E+00",
                    "module": "C1",
                    "scenario": null
                },
                {
                    "value": "0,00E+00",
                    "module": "C2",
                    "scenario": null
                },
                {
                    "value": "1,32E+00",
                    "module": "C3",
                    "scenario": null
                },
                {
                    "value": "2,31E-01",
                    "module": "C4",
                    "scenario": null
                },
                {
                    "value": "-6,42E-01",
                    "module": "D",
                    "scenario": null
                }
            ]
        },
        {
            "parameter": "PENRM",
            "values": [
                {
                    "value": "2,07E+01",
                    "module": "A1-A3",
                    "scenario": null
                },
                {
                    "value": "0,00E+00",
                    "module": "A4",
                    "scenario": null
                },
                {
                    "value": "0,00E+00",
                    "module": "A5",
                    "scenario": null
                },
                {
                    "value": "0,00E+00",
                    "module": "C1",
                    "scenario": null
                },
                {
                    "value": "0,00E+00",
                    "module": "C2",
                    "scenario": null
                },
                {
                    "value": "-2,07E+01",
                    "module": "C3",
                    "scenario": null
                },
                {
                    "value": "0,00E+00",
                    "module": "C4",
                    "scenario": null
                },
                {
                    "value": "0,00E+00",
                    "module": "D",
                    "scenario": null
                }
            ]
        },
        {
            "parameter": "PENRT",
            "values": [
                {
                    "value": "5,24E+01",
                    "module": "A1-A3",
                    "scenario": null
                },
                {
                    "value": "2,47E-01",
                    "module": "A4",
                    "scenario": null
                },
                {
                    "value": "0,00E+00",
                    "module": "A5",
                    "scenario": null
                },
                {
                    "value": "0,00E+00",
                    "module": "C1",
                    "scenario": null
                },
                {
                    "value": "0,00E+00",
                    "module": "C2",
                    "scenario": null
                },
                {
                    "value": "-1,94E+01",
                    "module": "C3",
                    "scenario": null
                },
                {
                    "value": "2,31E-01",
                    "module": "C4",
                    "scenario": null
                },
                {
                    "value": "-6,42E-01",
                    "module": "D",
                    "scenario": null
                }
            ]
        },
        {
            "parameter": "SM",
            "values": [
                {
                    "value": "0,00E+00",
                    "module": "A1-A3",
                    "scenario": null
                },
                {
                    "value": "0,00E+00",
                    "module": "A4",
                    "scenario": null
                },
                {
                    "value": "0,00E+00",
                    "module": "A5",
                    "scenario": null
                },
                {
                    "value": "0,00E+00",
                    "module": "C1",
                    "scenario": null
                },
                {
                    "value": "0,00E+00",
                    "module": "C2",
                    "scenario": null
                },
                {
                    "value": "0,00E+00",
                    "module": "C3",
                    "scenario": null
                },
                {
                    "value": "0,00E+00",
                    "module": "C4",
                    "scenario": null
                },
                {
                    "value": "0,00E+00",
                    "module": "D",
                    "scenario": null
                }
            ]
        },
        {
            "parameter": "RSF",
            "values": [
                {
                    "value": "1,57E-01",
                    "module": "A1-A3",
                    "scenario": null
                },
                {
                    "value": "1,26E-04",
                    "module": "A4",
                    "scenario": null
                },
                {
                    "value": "0,00E+00",
                    "module": "A5",
                    "scenario": null
                },
                {
                    "value": "0,00E+00",
                    "module": "C1",
                    "scenario": null
                },
                {
                    "value": "0,00E+00",
                    "module": "C2",
                    "scenario": null
                },
                {
                    "value": "3,04E-03",
                    "module": "C3",
                    "scenario": null
                },
                {
                    "value": "3,67E-04",
                    "module": "C4",
                    "scenario": null
                },
                {
                    "value": "-6,94E-04",
                    "module": "D",
                    "scenario": null
                }
            ]
        },
        {
            "parameter": "NRSF",
            "values": [
                {
                    "value": "2,13E-02",
                    "module": "A1-A3",
                    "scenario": null
                },
                {
                    "value": "4,52E-04",
                    "module": "A4",
                    "scenario": null
                },
                {
                    "value": "0,00E+00",
                    "module": "A5",
                    "scenario": null
                },
                {
                    "value": "0,00E+00",
                    "module": "C1",
                    "scenario": null
                },
                {
                    "value": "0,00E+00",
                    "module": "C2",
                    "scenario": null
                },
                {
                    "value": "0,00E+00",
                    "module": "C3",
                    "scenario": null
                },
                {
                    "value": "1,88E-03",
                    "module": "C4",
                    "scenario": null
                },
                {
                    "value": "-2,35E-01",
                    "module": "D",
                    "scenario": null
                }
            ]
        },
        {
            "parameter": "FW",
            "values": [
                {
                    "value": "3,57E-02",
                    "module": "A1-A3",
                    "scenario": null
                },
                {
                    "value": "2,64E-05",
                    "module": "A4",
                    "scenario": null
                },
                {
                    "value": "0,00E+00",
                    "module": "A5",
                    "scenario": null
                },
                {
                    "value": "0,00E+00",
                    "module": "C1",
                    "scenario": null
                },
                {
                    "value": "0,00E+00",
                    "module": "C2",
                    "scenario": null
                },
                {
                    "value": "3,15E-02",
                    "module": "C3",
                    "scenario": null
                },
                {
                    "value": "2,51E-04",
                    "module": "C4",
                    "scenario": null
                },
                {
                    "value": "-4,77E-03",
                    "module": "D",
                    "scenario": null
                }
            ]
        }
    ],
    "end_of_life_waste": [
        {
            "parameter": "HWD",
            "values": [
                {
                    "value": "4,94E-03",
                    "module": "A1-A3",
                    "scenario": null
                },
                {
                    "value": "1,27E-05",
                    "module": "A4",
                    "scenario": null
                },
                {
                    "value": "0,00E+00",
                    "module": "A5",
                    "scenario": null
                },
                {
                    "value": "0,00E+00",
                    "module": "C1",
                    "scenario": null
                },
                {
                    "value": "0,00E+00",
                    "module": "C2",
                    "scenario": null
                },
                {
                    "value": "0,00E+00",
                    "module": "C3",
                    "scenario": null
                },
                {
                    "value": "7,18E-03",
                    "module": "C4",
                    "scenario": null
                },
                {
                    "value": "-3,02E-05",
                    "module": "D",
                    "scenario": null
                }
            ]
        },
        {
            "parameter": "NHWD",
            "values": [
                {
                    "value": "2,98E-01",
                    "module": "A1-A3",
                    "scenario": null
                },
                {
                    "value": "1,20E-02",
                    "module": "A4",
                    "scenario": null
                },
                {
                    "value": "0,00E+00",
                    "module": "A5",
                    "scenario": null
                },
                {
                    "value": "0,00E+00",
                    "module": "C1",
                    "scenario": null
                },
                {
                    "value": "0,00E+00",
                    "module": "C2",
                    "scenario": null
                },
                {
                    "value": "0,00E+00",
                    "module": "C3",
                    "scenario": null
                },
                {
                    "value": "5,73E-01",
                    "module": "C4",
                    "scenario": null
                },
                {
                    "value": "-1,52E-02",
                    "module": "D",
                    "scenario": null
                }
            ]
        },
        {
            "parameter": "RWD",
            "values": [
                {
                    "value": "1,12E-04",
                    "module": "A1-A3",
                    "scenario": null
                },
                {
                    "value": "1,68E-06",
                    "module": "A4",
                    "scenario": null
                },
                {
                    "value": "0,00E+00",
                    "module": "A5",
                    "scenario": null
                },
                {
                    "value": "0,00E+00",
                    "module": "C1",
                    "scenario": null
                },
                {
                    "value": "0,00E+00",
                    "module": "C2",
                    "scenario": null
                },
                {
                    "value": "0,00E+00",
                    "module": "C3",
                    "scenario": null
                },
                {
                    "value": "1,03E-06",
                    "module": "C4",
                    "scenario": null
                },
                {
                    "value": "-3,36E-06",
                    "module": "D",
                    "scenario": null
                }
            ]
        }
    ],
    "end_of_life_flow": [
        {
            "parameter": "CRU",
            "values": [
                {
                    "value": "0,00E+00",
                    "module": "A1-A3",
                    "scenario": null
                },
                {
                    "value": "0,00E+00",
                    "module": "A4",
                    "scenario": null
                },
                {
                    "value": "0,00E+00",
                    "module": "A5",
                    "scenario": null
                },
                {
                    "value": "0,00E+00",
                    "module": "C1",
                    "scenario": null
                },
                {
                    "value": "0,00E+00",
                    "module": "C2",
                    "scenario": null
                },
                {
                    "value": "0,00E+00",
                    "module": "C3",
                    "scenario": null
                },
                {
                    "value": "0,00E+00",
                    "module": "C4",
                    "scenario": null
                },
                {
                    "value": "0,00E+00",
                    "module": "D",
                    "scenario": null
                }
            ]
        },
        {
            "parameter": "MFR",
            "values": [
                {
                    "value": "0,00E+00",
                    "module": "A1-A3",
                    "scenario": null
                },
                {
                    "value": "0,00E+00",
                    "module": "A4",
                    "scenario": null
                },
                {
                    "value": "0,00E+00",
                    "module": "A5",
                    "scenario": null
                },
                {
                    "value": "0,00E+00",
                    "module": "C1",
                    "scenario": null
                },
                {
                    "value": "0,00E+00",
                    "module": "C2",
                    "scenario": null
                },
                {
                    "value": "0,00E+00",
                    "module": "C3",
                    "scenario": null
                },
                {
                    "value": "4,48E-05",
                    "module": "C4",
                    "scenario": null
                },
                {
                    "value": "0,00E+00",
                    "module": "D",
                    "scenario": null
                }
            ]
        },
        {
            "parameter": "MER",
            "values": [
                {
                    "value": "0,00E+00",
                    "module": "A1-A3",
                    "scenario": null
                },
                {
                    "value": "0,00E+00",
                    "module": "A4",
                    "scenario": null
                },
                {
                    "value": "0,00E+00",
                    "module": "A5",
                    "scenario": null
                },
                {
                    "value": "0,00E+00",
                    "module": "C1",
                    "scenario": null
                },
                {
                    "value": "0,00E+00",
                    "module": "C2",
                    "scenario": null
                },
                {
                    "value": "5,00E-01",
                    "module": "C3",
                    "scenario": null
                },
                {
                    "value": "1,10E-06",
                    "module": "C4",
                    "scenario": null
                },
                {
                    "value": "0,00E+00",
                    "module": "D",
                    "scenario": null
                }
            ]
        },
        {
            "parameter": "EEE",
            "values": [
                {
                    "value": "0,00E+00",
                    "module": "A1-A3",
                    "scenario": null
                },
                {
                    "value": "0,00E+00",
                    "module": "A4",
                    "scenario": null
                },
                {
                    "value": "0,00E+00",
                    "module": "A5",
                    "scenario": null
                },
                {
                    "value": "0,00E+00",
                    "module": "C1",
                    "scenario": null
                },
                {
                    "value": "0,00E+00",
                    "module": "C2",
                    "scenario": null
                },
                {
                    "value": "5,11E-01",
                    "module": "C3",
                    "scenario": null
                },
                {
                    "value": "7,12E-05",
                    "module": "C4",
                    "scenario": null
                },
                {
                    "value": "0,00E+00",
                    "module": "D",
                    "scenario": null
                }
            ]
        },
        {
            "parameter": "EET",
            "values": [
                {
                    "value": "0,00E+00",
                    "module": "A1-A3",
                    "scenario": null
                },
                {
                    "value": "0,00E+00",
                    "module": "A4",
                    "scenario": null
                },
                {
                    "value": "0,00E+00",
                    "module": "A5",
                    "scenario": null
                },
                {
                    "value": "0,00E+00",
                    "module": "C1",
                    "scenario": null
                },
                {
                    "value": "0,00E+00",
                    "module": "C2",
                    "scenario": null
                },
                {
                    "value": "7,74E+00",
                    "module": "C3",
                    "scenario": null
                },
                {
                    "value": "1,08E-03",
                    "module": "C4",
                    "scenario": null
                },
                {
                    "value": "0,00E+00",
                    "module": "D",
                    "scenario": null
                }
            ]
        }
    ]
}