{
    "product_name": "Component EPD Surnadal: PVC insulated and PVC sheathed house wiring cable for open, fixed installation indoors and outdoors PR 2x1,5/1,5",
    "epd_id": "NEPD-8141-7805",
    "compliance": [
        "EN 15804+A2",
        "ISO 14025",
        "ISO 21930"
    ],
    "producer_name": "Pipelife Norge AS",
    "environmental_impact": [
        {
            "parameter": "GWP-total",
            "values": [
                {
                    "value": "3,91E+00",
                    "module": "A1-A3",
                    "scenario": null
                },
                {
                    "value": "1,63E-02",
                    "module": "A4",
                    "scenario": null
                },
                {
                    "value": "0,00E+00",
                    "module": "C1",
                    "scenario": null
                },
                {
                    "value": "0,00E+00",
                    "module": "C2",
                    "scenario": null
                },
                {
                    "value": "0,00E+00",
                    "module": "C3",
                    "scenario": null
                },
                {
                    "value": "0,00E+00",
                    "module": "C4",
                    "scenario": null
                },
                {
                    "value": "0,00E+00",
                    "module": "D",
                    "scenario": null
                }
            ]
        },
        {
            "parameter": "GWP-fossil",
            "values": [
                {
                    "value": "3,88E+00",
                    "module": "A1-A3",
                    "scenario": null
                },
                {
                    "value": "1,63E-02",
                    "module": "A4",
                    "scenario": null
                },
                {
                    "value": "0,00E+00",
                    "module": "C1",
                    "scenario": null
                },
                {
                    "value": "0,00E+00",
                    "module": "C2",
                    "scenario": null
                },
                {
                    "value": "0,00E+00",
                    "module": "C3",
                    "scenario": null
                },
                {
                    "value": "0,00E+00",
                    "module": "C4",
                    "scenario": null
                },
                {
                    "value": "0,00E+00",
                    "module": "D",
                    "scenario": null
                }
            ]
        },
        {
            "parameter": "GWP-biogenic",
            "values": [
                {
                    "value": "2,10E-02",
                    "module": "A1-A3",
                    "scenario": null
                },
                {
                    "value": "6,76E-06",
                    "module": "A4",
                    "scenario": null
                },
                {
                    "value": "0,00E+00",
                    "module": "C1",
                    "scenario": null
                },
                {
                    "value": "0,00E+00",
                    "module": "C2",
                    "scenario": null
                },
                {
                    "value": "0,00E+00",
                    "module": "C3",
                    "scenario": null
                },
                {
                    "value": "0,00E+00",
                    "module": "C4",
                    "scenario": null
                },
                {
                    "value": "0,00E+00",
                    "module": "D",
                    "scenario": null
                }
            ]
        },
        {
            "parameter": "GWP-luluc",
            "values": [
                {
                    "value": "1,10E-02",
                    "module": "A1-A3",
                    "scenario": null
                },
                {
                    "value": "5,81E-06",
                    "module": "A4",
                    "scenario": null
                },
                {
                    "value": "0,00E+00",
                    "module": "C1",
                    "scenario": null
                },
                {
                    "value": "0,00E+00",
                    "module": "C2",
                    "scenario": null
                },
                {
                    "value": "0,00E+00",
                    "module": "C3",
                    "scenario": null
                },
                {
                    "value": "0,00E+00",
                    "module": "C4",
                    "scenario": null
                },
                {
                    "value": "0,00E+00",
                    "module": "D",
                    "scenario": null
                }
            ]
        },
        {
            "parameter": "ODP",
            "values": [
                {
                    "value": "3,71E-08",
                    "module": "A1-A3",
                    "scenario": null
                },
                {
                    "value": "3,70E-09",
                    "module": "A4",
                    "scenario": null
                },
                {
                    "value": "0,00E+00",
                    "module": "C1",
                    "scenario": null
                },
                {
                    "value": "0,00E+00",
                    "module": "C2",
                    "scenario": null
                },
                {
                    "value": "0,00E+00",
                    "module": "C3",
                    "scenario": null
                },
                {
                    "value": "0,00E+00",
                    "module": "C4",
                    "scenario": null
                },
                {
                    "value": "0,00E+00",
                    "module": "D",
                    "scenario": null
                }
            ]
        },
        {
            "parameter": "AP",
            "values": [
                {
                    "value": "3,73E-02",
                    "module": "A1-A3",
                    "scenario": null
                },
                {
                    "value": "4,69E-05",
                    "module": "A4",
                    "scenario": null
                },
                {
                    "value": "0,00E+00",
                    "module": "C1",
                    "scenario": null
                },
                {
                    "value": "0,00E+00",
                    "module": "C2",
                    "scenario": null
                },
                {
                    "value": "0,00E+00",
                    "module": "C3",
                    "scenario": null
                },
                {
                    "value": "0,00E+00",
                    "module": "C4",
                    "scenario": null
                },
                {
                    "value": "0,00E+00",
                    "module": "D",
                    "scenario": null
                }
            ]
        },
        {
            "parameter": "POCP",
            "values": [
                {
                    "value": "1,11E-02",
                    "module": "A1-A3",
                    "scenario": null
                },
                {
                    "value": "3,98E-05",
                    "module": "A4",
                    "scenario": null
                },
                {
                    "value": "0,00E+00",
                    "module": "C1",
                    "scenario": null
                },
                {
                    "value": "0,00E+00",
                    "module": "C2",
                    "scenario": null
                },
                {
                    "value": "0,00E+00",
                    "module": "C3",
                    "scenario": null
                },
                {
                    "value": "0,00E+00",
                    "module": "C4",
                    "scenario": null
                },
                {
                    "value": "0,00E+00",
                    "module": "D",
                    "scenario": null
                }
            ]
        },
        {
            "parameter": "ADPE",
            "values": [
                {
                    "value": "1,40E-03",
                    "module": "A1-A3",
                    "scenario": null
                },
                {
                    "value": "4,51E-07",
                    "module": "A4",
                    "scenario": null
                },
                {
                    "value": "0,00E+00",
                    "module": "C1",
                    "scenario": null
                },
                {
                    "value": "0,00E+00",
                    "module": "C2",
                    "scenario": null
                },
                {
                    "value": "0,00E+00",
                    "module": "C3",
                    "scenario": null
                },
                {
                    "value": "0,00E+00",
                    "module": "C4",
                    "scenario": null
                },
                {
                    "value": "0,00E+00",
                    "module": "D",
                    "scenario": null
                }
            ]
        },
        {
            "parameter": "ADPF",
            "values": [
                {
                    "value": "6,48E+01",
                    "module": "A1-A3",
                    "scenario": null
                },
                {
                    "value": "2,47E-01",
                    "module": "A4",
                    "scenario": null
                },
                {
                    "value": "0,00E+00",
                    "module": "C1",
                    "scenario": null
                },
                {
                    "value": "0,00E+00",
                    "module": "C2",
                    "scenario": null
                },
                {
                    "value": "0,00E+00",
                    "module": "C3",
                    "scenario": null
                },
                {
                    "value": "0,00E+00",
                    "module": "C4",
                    "scenario": null
                },
                {
                    "value": "0,00E+00",
                    "module": "D",
                    "scenario": null
                }
            ]
        },
        {
            "parameter": "WDP",
            "values": [
                {
                    "value": "3,51E+00",
                    "module": "A1-A3",
                    "scenario": null
                },
                {
                    "value": "2,39E-01",
                    "module": "A4",
                    "scenario": null
                },
                {
                    "value": "0,00E+00",
                    "module": "C1",
                    "scenario": null
                },
                {
                    "value": "0,00E+00",
                    "module": "C2",
                    "scenario": null
                },
                {
                    "value": "0,00E+00",
                    "module": "C3",
                    "scenario": null
                },
                {
                    "value": "0,00E+00",
                    "module": "C4",
                    "scenario": null
                },
                {
                    "value": "0,00E+00",
                    "module": "D",
                    "scenario": null
                }
            ]
        },
        {
            "parameter": "EP-freshwater",
            "values": [
                {
                    "value": "9,58E-06",
                    "module": "A1-A3",
                    "scenario": null
                },
                {
                    "value": "1,31E-07",
                    "module": "A4",
                    "scenario": null
                },
                {
                    "value": "0,00E+00",
                    "module": "C1",
                    "scenario": null
                },
                {
                    "value": "0,00E+00",
                    "module": "C2",
                    "scenario": null
                },
                {
                    "value": "0,00E+00",
                    "module": "C3",
                    "scenario": null
                },
                {
                    "value": "0,00E+00",
                    "module": "C4",
                    "scenario": null
                },
                {
                    "value": "0,00E+00",
                    "module": "D",
                    "scenario": null
                }
            ]
        },
        {
            "parameter": "EP-marine",
            "values": [
                {
                    "value": "2,95E-03",
                    "module": "A1-A3",
                    "scenario": null
                },
                {
                    "value": "9,29E-06",
                    "module": "A4",
                    "scenario": null
                },
                {
                    "value": "0,00E+00",
                    "module": "C1",
                    "scenario": null
                },
                {
                    "value": "0,00E+00",
                    "module": "C2",
                    "scenario": null
                },
                {
                    "value": "0,00E+00",
                    "module": "C3",
                    "scenario": null
                },
                {
                    "value": "0,00E+00",
                    "module": "C4",
                    "scenario": null
                },
                {
                    "value": "0,00E+00",
                    "module": "D",
                    "scenario": null
                }
            ]
        },
        {
            "parameter": "EP-terrestrial",
            "values": [
                {
                    "value": "3,11E-02",
                    "module": "A1-A3",
                    "scenario": null
                },
                {
                    "value": "1,04E-04",
                    "module": "A4",
                    "scenario": null
                },
                {
                    "value": "0,00E+00",
                    "module": "C1",
                    "scenario": null
                },
                {
                    "value": "0,00E+00",
                    "module": "C2",
                    "scenario": null
                },
                {
                    "value": "0,00E+00",
                    "module": "C3",
                    "scenario": null
                },
                {
                    "value": "0,00E+00",
                    "module": "C4",
                    "scenario": null
                },
                {
                    "value": "0,00E+00",
                    "module": "D",
                    "scenario": null
                }
            ]
        },
        {
            "parameter": "GWP-IOBC",
            "values": [
                {
                    "value": "3,83E+00",
                    "module": "A1-A3",
                    "scenario": null
                },
                {
                    "value": "1,63E-02",
                    "module": "A4",
                    "scenario": null
                },
                {
                    "value": "0,00E+00",
                    "module": "C1",
                    "scenario": null
                },
                {
                    "value": "0,00E+00",
                    "module": "C2",
                    "scenario": null
                },
                {
                    "value": "0,00E+00",
                    "module": "C3",
                    "scenario": null
                },
                {
                    "value": "0,00E+00",
                    "module": "C4",
                    "scenario": null
                },
                {
                    "value": "0,00E+00",
                    "module": "D",
                    "scenario": null
                }
            ]
        }
    ],
    "additional_environmental_impact": [
        {
            "parameter": "PM",
            "values": [
                {
                    "value": "1,00E-08",
                    "module": "A1-A3",
                    "scenario": null
                },
                {
                    "value": "1,00E-09",
                    "module": "A4",
                    "scenario": null
                },
                {
                    "value": "0,00E+00",
                    "module": "C1",
                    "scenario": null
                },
                {
                    "value": "0,00E+00",
                    "module": "C2",
                    "scenario": null
                },
                {
                    "value": "0,00E+00",
                    "module": "C3",
                    "scenario": null
                },
                {
                    "value": "0,00E+00",
                    "module": "C4",
                    "scenario": null
                },
                {
                    "value": "0,00E+00",
                    "module": "D",
                    "scenario": null
                }
            ]
        },
        {
            "parameter": "ETP-fw",
            "values": [
                {
                    "value": "1,83E+00",
                    "module": "A1-A3",
                    "scenario": null
                },
                {
                    "value": "1,83E-01",
                    "module": "A4",
                    "scenario": null
                },
                {
                    "value": "0,00E+00",
                    "module": "C1",
                    "scenario": null
                },
                {
                    "value": "0,00E+00",
                    "module": "C2",
                    "scenario": null
                },
                {
                    "value": "0,00E+00",
                    "module": "C3",
                    "scenario": null
                },
                {
                    "value": "0,00E+00",
                    "module": "C4",
                    "scenario": null
                },
                {
                    "value": "0,00E+00",
                    "module": "D",
                    "scenario": null
                }
            ]
        },
        {
            "parameter": "HTP-c",
            "values": [
                {
                    "value": "0,00E+00",
                    "module": "A1-A3",
                    "scenario": null
                },
                {
                    "value": "0,00E+00",
                    "module": "A4",
                    "scenario": null
                },
                {
                    "value": "0,00E+00",
                    "module": "C1",
                    "scenario": null
                },
                {
                    "value": "0,00E+00",
                    "module": "C2",
                    "scenario": null
                },
                {
                    "value": "0,00E+00",
                    "module": "C3",
                    "scenario": null
                },
                {
                    "value": "0,00E+00",
                    "module": "C4",
                    "scenario": null
                },
                {
                    "value": "0,00E+00",
                    "module": "D",
                    "scenario": null
                }
            ]
        },
        {
            "parameter": "HTP-nc",
            "values": [
                {
                    "value": "2,00E-09",
                    "module": "A1-A3",
                    "scenario": null
                },
                {
                    "value": "2,00E-10",
                    "module": "A4",
                    "scenario": null
                },
                {
                    "value": "0,00E+00",
                    "module": "C1",
                    "scenario": null
                },
                {
                    "value": "0,00E+00",
                    "module": "C2",
                    "scenario": null
                },
                {
                    "value": "0,00E+00",
                    "module": "C3",
                    "scenario": null
                },
                {
                    "value": "0,00E+00",
                    "module": "C4",
                    "scenario": null
                },
                {
                    "value": "0,00E+00",
                    "module": "D",
                    "scenario": null
                }
            ]
        },
        {
            "parameter": "SQP",
            "values": [
                {
                    "value": "1,73E+00",
                    "module": "A1-A3",
                    "scenario": null
                },
                {
                    "value": "1,73E-01",
                    "module": "A4",
                    "scenario": null
                },
                {
                    "value": "0,00E+00",
                    "module": "C1",
                    "scenario": null
                },
                {
                    "value": "0,00E+00",
                    "module": "C2",
                    "scenario": null
                },
                {
                    "value": "0,00E+00",
                    "module": "C3",
                    "scenario": null
                },
                {
                    "value": "0,00E+00",
                    "module": "C4",
                    "scenario": null
                },
                {
                    "value": "0,00E+00",
                    "module": "D",
                    "scenario": null
                }
            ]
        },
        {
            "parameter": "IRP",
            "values": [
                {
                    "value": "1,08E-02",
                    "module": "A1-A3",
                    "scenario": null
                },
                {
                    "value": "1,08E-03",
                    "module": "A4",
                    "scenario": null
                },
                {
                    "value": "0,00E+00",
                    "module": "C1",
                    "scenario": null
                },
                {
                    "value": "0,00E+00",
                    "module": "C2",
                    "scenario": null
                },
                {
                    "value": "0,00E+00",
                    "module": "C3",
                    "scenario": null
                },
                {
                    "value": "0,00E+00",
                    "module": "C4",
                    "scenario": null
                },
                {
                    "value": "0,00E+00",
                    "module": "D",
                    "scenario": null
                }
            ]
        }
    ],
    "resource_use": [
        {
            "parameter": "PERE",
            "values": [
                {
                    "value": "1,14E+01",
                    "module": "A1-A3",
                    "scenario": null
                },
                {
                    "value": "3,54E-03",
                    "module": "A4",
                    "scenario": null
                },
                {
                    "value": "0,00E+00",
                    "module": "C1",
                    "scenario": null
                },
                {
                    "value": "0,00E+00",
                    "module": "C2",
                    "scenario": null
                },
                {
                    "value": "0,00E+00",
                    "module": "C3",
                    "scenario": null
                },
                {
                    "value": "0,00E+00",
                    "module": "C4",
                    "scenario": null
                },
                {
                    "value": "0,00E+00",
                    "module": "D",
                    "scenario": null
                }
            ]
        },
        {
            "parameter": "PERM",
            "values": [
                {
                    "value": "0,00E+00",
                    "module": "A1-A3",
                    "scenario": null
                },
                {
                    "value": "0,00E+00",
                    "module": "A4",
                    "scenario": null
                },
                {
                    "value": "0,00E+00",
                    "module": "C1",
                    "scenario": null
                },
                {
                    "value": "0,00E+00",
                    "module": "C2",
                    "scenario": null
                },
                {
                    "value": "0,00E+00",
                    "module": "C3",
                    "scenario": null
                },
                {
                    "value": "0,00E+00",
                    "module": "C4",
                    "scenario": null
                },
                {
                    "value": "0,00E+00",
                    "module": "D",
                    "scenario": null
                }
            ]
        },
        {
            "parameter": "PERT",
            "values": [
                {
                    "value": "1,14E+01",
                    "module": "A1-A3",
                    "scenario": null
                },
                {
                    "value": "3,54E-03",
                    "module": "A4",
                    "scenario": null
                },
                {
                    "value": "0,00E+00",
                    "module": "C1",
                    "scenario": null
                },
                {
                    "value": "0,00E+00",
                    "module": "C2",
                    "scenario": null
                },
                {
                    "value": "0,00E+00",
                    "module": "C3",
                    "scenario": null
                },
                {
                    "value": "0,00E+00",
                    "module": "C4",
                    "scenario": null
                },
                {
                    "value": "0,00E+00",
                    "module": "D",
                    "scenario": null
                }
            ]
        },
        {
            "parameter": "PENRE",
            "values": [
                {
                    "value": "5,30E+01",
                    "module": "A1-A3",
                    "scenario": null
                },
                {
                    "value": "2,47E-01",
                    "module": "A4",
                    "scenario": null
                },
                {
                    "value": "0,00E+00",
                    "module": "C1",
                    "scenario": null
                },
                {
                    "value": "0,00E+00",
                    "module": "C2",
                    "scenario": null
                },
                {
                    "value": "0,00E+00",
                    "module": "C3",
                    "scenario": null
                },
                {
                    "value": "0,00E+00",
                    "module": "C4",
                    "scenario": null
                },
                {
                    "value": "0,00E+00",
                    "module": "D",
                    "scenario": null
                }
            ]
        },
        {
            "parameter": "PENRM",
            "values": [
                {
                    "value": "1,15E+01",
                    "module": "A1-A3",
                    "scenario": null
                },
                {
                    "value": "0,00E+00",
                    "module": "A4",
                    "scenario": null
                },
                {
                    "value": "0,00E+00",
                    "module": "C1",
                    "scenario": null
                },
                {
                    "value": "0,00E+00",
                    "module": "C2",
                    "scenario": null
                },
                {
                    "value": "0,00E+00",
                    "module": "C3",
                    "scenario": null
                },
                {
                    "value": "0,00E+00",
                    "module": "C4",
                    "scenario": null
                },
                {
                    "value": "0,00E+00",
                    "module": "D",
                    "scenario": null
                }
            ]
        },
        {
            "parameter": "PENRT",
            "values": [
                {
                    "value": "6,45E+01",
                    "module": "A1-A3",
                    "scenario": null
                },
                {
                    "value": "2,47E-01",
                    "module": "A4",
                    "scenario": null
                },
                {
                    "value": "0,00E+00",
                    "module": "C1",
                    "scenario": null
                },
                {
                    "value": "0,00E+00",
                    "module": "C2",
                    "scenario": null
                },
                {
                    "value": "0,00E+00",
                    "module": "C3",
                    "scenario": null
                },
                {
                    "value": "0,00E+00",
                    "module": "C4",
                    "scenario": null
                },
                {
                    "value": "0,00E+00",
                    "module": "D",
                    "scenario": null
                }
            ]
        },
        {
            "parameter": "SM",
            "values": [
                {
                    "value": "0,00E+00",
                    "module": "A1-A3",
                    "scenario": null
                },
                {
                    "value": "0,00E+00",
                    "module": "A4",
                    "scenario": null
                },
                {
                    "value": "0,00E+00",
                    "module": "C1",
                    "scenario": null
                },
                {
                    "value": "0,00E+00",
                    "module": "C2",
                    "scenario": null
                },
                {
                    "value": "0,00E+00",
                    "module": "C3",
                    "scenario": null
                },
                {
                    "value": "0,00E+00",
                    "module": "C4",
                    "scenario": null
                },
                {
                    "value": "0,00E+00",
                    "module": "D",
                    "scenario": null
                }
            ]
        },
        {
            "parameter": "RSF",
            "values": [
                {
                    "value": "1,27E-03",
                    "module": "A1-A3",
                    "scenario": null
                },
                {
                    "value": "1,26E-04",
                    "module": "A4",
                    "scenario": null
                },
                {
                    "value": "0,00E+00",
                    "module": "C1",
                    "scenario": null
                },
                {
                    "value": "0,00E+00",
                    "module": "C2",
                    "scenario": null
                },
                {
                    "value": "0,00E+00",
                    "module": "C3",
                    "scenario": null
                },
                {
                    "value": "0,00E+00",
                    "module": "C4",
                    "scenario": null
                },
                {
                    "value": "0,00E+00",
                    "module": "D",
                    "scenario": null
                }
            ]
        },
        {
            "parameter": "NRSF",
            "values": [
                {
                    "value": "4,53E-03",
                    "module": "A1-A3",
                    "scenario": null
                },
                {
                    "value": "4,52E-04",
                    "module": "A4",
                    "scenario": null
                },
                {
                    "value": "0,00E+00",
                    "module": "C1",
                    "scenario": null
                },
                {
                    "value": "0,00E+00",
                    "module": "C2",
                    "scenario": null
                },
                {
                    "value": "0,00E+00",
                    "module": "C3",
                    "scenario": null
                },
                {
                    "value": "0,00E+00",
                    "module": "C4",
                    "scenario": null
                },
                {
                    "value": "0,00E+00",
                    "module": "D",
                    "scenario": null
                }
            ]
        },
        {
            "parameter": "FW",
            "values": [
                {
                    "value": "3,60E-02",
                    "module": "A1-A3",
                    "scenario": null
                },
                {
                    "value": "2,64E-05",
                    "module": "A4",
                    "scenario": null
                },
                {
                    "value": "0,00E+00",
                    "module": "C1",
                    "scenario": null
                },
                {
                    "value": "0,00E+00",
                    "module": "C2",
                    "scenario": null
                },
                {
                    "value": "0,00E+00",
                    "module": "C3",
                    "scenario": null
                },
                {
                    "value": "0,00E+00",
                    "module": "C4",
                    "scenario": null
                },
                {
                    "value": "0,00E+00",
                    "module": "D",
                    "scenario": null
                }
            ]
        }
    ],
    "end_of_life_waste": [
        {
            "parameter": "HWD",
            "values": [
                {
                    "value": "1,28E-04",
                    "module": "A1-A3",
                    "scenario": null
                },
                {
                    "value": "1,27E-05",
                    "module": "A4",
                    "scenario": null
                },
                {
                    "value": "0,00E+00",
                    "module": "C1",
                    "scenario": null
                },
                {
                    "value": "0,00E+00",
                    "module": "C2",
                    "scenario": null
                },
                {
                    "value": "0,00E+00",
                    "module": "C3",
                    "scenario": null
                },
                {
                    "value": "0,00E+00",
                    "module": "C4",
                    "scenario": null
                },
                {
                    "value": "0,00E+00",
                    "module": "D",
                    "scenario": null
                }
            ]
        },
        {
            "parameter": "NHWD",
            "values": [
                {
                    "value": "1,41E-01",
                    "module": "A1-A3",
                    "scenario": null
                },
                {
                    "value": "1,20E-02",
                    "module": "A4",
                    "scenario": null
                },
                {
                    "value": "0,00E+00",
                    "module": "C1",
                    "scenario": null
                },
                {
                    "value": "0,00E+00",
                    "module": "C2",
                    "scenario": null
                },
                {
                    "value": "0,00E+00",
                    "module": "C3",
                    "scenario": null
                },
                {
                    "value": "0,00E+00",
                    "module": "C4",
                    "scenario": null
                },
                {
                    "value": "0,00E+00",
                    "module": "D",
                    "scenario": null
                }
            ]
        },
        {
            "parameter": "RWD",
            "values": [
                {
                    "value": "1,69E-05",
                    "module": "A1-A3",
                    "scenario": null
                },
                {
                    "value": "1,68E-06",
                    "module": "A4",
                    "scenario": null
                },
                {
                    "value": "0,00E+00",
                    "module": "C1",
                    "scenario": null
                },
                {
                    "value": "0,00E+00",
                    "module": "C2",
                    "scenario": null
                },
                {
                    "value": "0,00E+00",
                    "module": "C3",
                    "scenario": null
                },
                {
                    "value": "0,00E+00",
                    "module": "C4",
                    "scenario": null
                },
                {
                    "value": "0,00E+00",
                    "module": "D",
                    "scenario": null
                }
            ]
        }
    ],
    "end_of_life_flow": [
        {
            "parameter": "CRU",
            "values": [
                {
                    "value": "0,00E+00",
                    "module": "A1-A3",
                    "scenario": null
                },
                {
                    "value": "0,00E+00",
                    "module": "A4",
                    "scenario": null
                },
                {
                    "value": "0,00E+00",
                    "module": "C1",
                    "scenario": null
                },
                {
                    "value": "0,00E+00",
                    "module": "C2",
                    "scenario": null
                },
                {
                    "value": "0,00E+00",
                    "module": "C3",
                    "scenario": null
                },
                {
                    "value": "0,00E+00",
                    "module": "C4",
                    "scenario": null
                },
                {
                    "value": "0,00E+00",
                    "module": "D",
                    "scenario": null
                }
            ]
        },
        {
            "parameter": "MFR",
            "values": [
                {
                    "value": "0,00E+00",
                    "module": "A1-A3",
                    "scenario": null
                },
                {
                    "value": "0,00E+00",
                    "module": "A4",
                    "scenario": null
                },
                {
                    "value": "0,00E+00",
                    "module": "C1",
                    "scenario": null
                },
                {
                    "value": "0,00E+00",
                    "module": "C2",
                    "scenario": null
                },
                {
                    "value": "0,00E+00",
                    "module": "C3",
                    "scenario": null
                },
                {
                    "value": "0,00E+00",
                    "module": "C4",
                    "scenario": null
                },
                {
                    "value": "0,00E+00",
                    "module": "D",
                    "scenario": null
                }
            ]
        },
        {
            "parameter": "MER",
            "values": [
                {
                    "value": "0,00E+00",
                    "module": "A1-A3",
                    "scenario": null
                },
                {
                    "value": "0,00E+00",
                    "module": "A4",
                    "scenario": null
                },
                {
                    "value": "0,00E+00",
                    "module": "C1",
                    "scenario": null
                },
                {
                    "value": "0,00E+00",
                    "module": "C2",
                    "scenario": null
                },
                {
                    "value": "0,00E+00",
                    "module": "C3",
                    "scenario": null
                },
                {
                    "value": "0,00E+00",
                    "module": "C4",
                    "scenario": null
                },
                {
                    "value": "0,00E+00",
                    "module": "D",
                    "scenario": null
                }
            ]
        },
        {
            "parameter": "EEE",
            "values": [
                {
                    "value": "0,00E+00",
                    "module": "A1-A3",
                    "scenario": null
                },
                {
                    "value": "0,00E+00",
                    "module": "A4",
                    "scenario": null
                },
                {
                    "value": "0,00E+00",
                    "module": "C1",
                    "scenario": null
                },
                {
                    "value": "0,00E+00",
                    "module": "C2",
                    "scenario": null
                },
                {
                    "value": "0,00E+00",
                    "module": "C3",
                    "scenario": null
                },
                {
                    "value": "0,00E+00",
                    "module": "C4",
                    "scenario": null
                },
                {
                    "value": "0,00E+00",
                    "module": "D",
                    "scenario": null
                }
            ]
        },
        {
            "parameter": "EET",
            "values": [
                {
                    "value": "0,00E+00",
                    "module": "A1-A3",
                    "scenario": null
                },
                {
                    "value": "0,00E+00",
                    "module": "A4",
                    "scenario": null
                },
                {
                    "value": "0,00E+00",
                    "module": "C1",
                    "scenario": null
                },
                {
                    "value": "0,00E+00",
                    "module": "C2",
                    "scenario": null
                },
                {
                    "value": "0,00E+00",
                    "module": "C3",
                    "scenario": null
                },
                {
                    "value": "0,00E+00",
                    "module": "C4",
                    "scenario": null
                },
                {
                    "value": "0,00E+00",
                    "module": "D",
                    "scenario": null
                }
            ]
        }
    ]
}