{"product_name":"Cold-formed welded structural hollow sections of non-alloy and fine grains steels ","epd_id":"DAP012:2024","compliance":["EN 15804+A2","ISO 14025"],"producer_name":"Ferpinta \u2013 Ind\u00fastrias de Tubos de A\u00e7o de Fernando Pinho Teixeira, S.A.","environmental_impact":[{"parameter":"GWP-total","unit":"kg CO2-eq.","values":[{"value":"1,81E+03","module":"A1-A3"},{"value":"2,44E+01","module":"C2"},{"value":"1,26E+01","module":"C3"},{"value":"0,0E+00","module":"C4"},{"value":"-8,70E+02","module":"D"}]},{"parameter":"GWP-fossil","unit":"kg CO2-eq.","values":[{"value":"1,80E+03","module":"A1-A3"},{"value":"2,44E+01","module":"C2"},{"value":"1,24E+01","module":"C3"},{"value":"0,0E+00","module":"C4"},{"value":"-8,60E+02","module":"D"}]},{"parameter":"GWP-biogenic","unit":"kg CO2-eq.","values":[{"value":"1,42E+01","module":"A1-A3"},{"value":"1,34E-02","module":"C2"},{"value":"1,66E-01","module":"C3"},{"value":"0,0E+00","module":"C4"},{"value":"-1,12E+01","module":"D"}]},{"parameter":"GWP-luluc","unit":"kg CO2-eq.","values":[{"value":"1,10E+00","module":"A1-A3"},{"value":"4,65E-04","module":"C2"},{"value":"2,04E-02","module":"C3"},{"value":"0,0E+00","module":"C4"},{"value":"2,90E-01","module":"D"}]},{"parameter":"ODP","unit":"kg CFC 11-equiv.","values":[{"value":"3,42E-05","module":"A1-A3"},{"value":"5,04E-07","module":"C2"},{"value":"2,09E-07","module":"C3"},{"value":"0,0E+00","module":"C4"},{"value":"-1,70E-05","module":"D"}]},{"parameter":"AP","unit":"mol H+-eq.","values":[{"value":"9,93E+00","module":"A1-A3"},{"value":"5,99E-02","module":"C2"},{"value":"1,02E-01","module":"C3"},{"value":"0,0E+00","module":"C4"},{"value":"-3,40E+00","module":"D"}]},{"parameter":"POCP","unit":"kg NMVOC-eq.","values":[{"value":"9,79E+00","module":"A1-A3"},{"value":"9,67E-02","module":"C2"},{"value":"1,42E-01","module":"C3"},{"value":"0,0E+00","module":"C4"},{"value":"-4,24E+00","module":"D"}]},{"parameter":"ADPE","unit":"kg Sb-eq.","values":[{"value":"6,11E-03","module":"A1-A3"},{"value":"8,15E-07","module":"C2"},{"value":"5,36E-07","module":"C3"},{"value":"0,0E+00","module":"C4"},{"value":"-7,66E-03","module":"D"}]},{"parameter":"ADPF","unit":"MJ","values":[{"value":"2,00E+04","module":"A1-A3"},{"value":"3,12E+02","module":"C2"},{"value":"1,93E+02","module":"C3"},{"value":"0,0E+00","module":"C4"},{"value":"-7,51E+03","module":"D"}]},{"parameter":"WDP","unit":"m3 world-eq.","values":[{"value":"1,05E+02","module":"A1-A3"},{"value":"2,89E-01","module":"C2"},{"value":"1,33E+00","module":"C3"},{"value":"0,0E+00","module":"C4"},{"value":"-8,03E+01","module":"D"}]},{"parameter":"EP-freshwater","unit":"kg P-eq.","values":[{"value":"1,09E-01","module":"A1-A3"},{"value":"1,90E-05","module":"C2"},{"value":"1,16E-04","module":"C3"},{"value":"0,0E+00","module":"C4"},{"value":"-4,07E-02","module":"D"}]},{"parameter":"EP-marine","unit":"kg N-eq.","values":[{"value":"2,05E+00","module":"A1-A3"},{"value":"2,33E-02","module":"C2"},{"value":"4,41E-02","module":"C3"},{"value":"0,0E+00","module":"C4"},{"value":"-6,87E-01","module":"D"}]},{"parameter":"EP-terrestrial","unit":"mol N-eq.","values":[{"value":"2,23E+01","module":"A1-A3"},{"value":"2,45E-01","module":"C2"},{"value":"4,80E-01","module":"C3"},{"value":"0,0E+00","module":"C4"},{"value":"-7,96E+00","module":"D"}]}],"additional_environmental_impact":[{"parameter":"PM","unit":"disease incidence","values":[{"value":null,"module":"A1-A3"},{"value":null,"module":"C2"},{"value":null,"module":"C3"},{"value":null,"module":"C4"},{"value":null,"module":"D"}]},{"parameter":"ETP-fw","unit":"CTUe","values":[{"value":null,"module":"A1-A3"},{"value":null,"module":"C2"},{"value":null,"module":"C3"},{"value":null,"module":"C4"},{"value":null,"module":"D"}]},{"parameter":"HTP-c","unit":"CTUh","values":[{"value":null,"module":"A1-A3"},{"value":null,"module":"C2"},{"value":null,"module":"C3"},{"value":null,"module":"C4"},{"value":null,"module":"D"}]},{"parameter":"HTP-nc","unit":"CTUh","values":[{"value":null,"module":"A1-A3"},{"value":null,"module":"C2"},{"value":null,"module":"C3"},{"value":null,"module":"C4"},{"value":null,"module":"D"}]},{"parameter":"SQP","unit":"dimensionless","values":[{"value":null,"module":"A1-A3"},{"value":null,"module":"C2"},{"value":null,"module":"C3"},{"value":null,"module":"C4"},{"value":null,"module":"D"}]},{"parameter":"IRP","unit":"kBq U235-eq.","values":[{"value":null,"module":"A1-A3"},{"value":null,"module":"C2"},{"value":null,"module":"C3"},{"value":null,"module":"C4"},{"value":null,"module":"D"}]}],"resource_use":[{"parameter":"PERE","unit":"MJ","values":[{"value":"1,35E+03","module":"A1-A3"},{"value":"8,14E-01","module":"C2"},{"value":"1,69E+01","module":"C3"},{"value":"0,0E+00","module":"C4"},{"value":"-4,47E+02","module":"D"}]},{"parameter":"PERM","unit":"MJ","values":[{"value":"5,39E+01","module":"A1-A3"},{"value":"0,0E+00","module":"C2"},{"value":"0,0E+00","module":"C3"},{"value":"0,0E+00","module":"C4"},{"value":"0,0E+00","module":"D"}]},{"parameter":"PERT","unit":"MJ","values":[{"value":"1,40E+03","module":"A1-A3"},{"value":"8,14E-01","module":"C2"},{"value":"1,69E+01","module":"C3"},{"value":"0,0E+00","module":"C4"},{"value":"-4,47E+02","module":"D"}]},{"parameter":"PENRE","unit":"MJ","values":[{"value":"1,99E+04","module":"A1-A3"},{"value":"3,12E+02","module":"C2"},{"value":"1,93E+02","module":"C3"},{"value":"0,0E+00","module":"C4"},{"value":"-7,51E+03","module":"D"}]},{"parameter":"PENRM","unit":"MJ","values":[{"value":"4,56E+01","module":"A1-A3"},{"value":"0,0E+00","module":"C2"},{"value":"0,0E+00","module":"C3"},{"value":"0,0E+00","module":"C4"},{"value":"0,0E+00","module":"D"}]},{"parameter":"PENRT","unit":"MJ","values":[{"value":"2,00E+04","module":"A1-A3"},{"value":"3,12E+02","module":"C2"},{"value":"1,93E+02","module":"C3"},{"value":"0,0E+00","module":"C4"},{"value":"-7,51E+03","module":"D"}]},{"parameter":"SM","unit":"kg","values":[{"value":"4,37E+02","module":"A1-A3"},{"value":"0,0E+00","module":"C2"},{"value":"0,0E+00","module":"C3"},{"value":"0,0E+00","module":"C4"},{"value":"6,01E+02","module":"D"}]},{"parameter":"RSF","unit":"MJ","values":[{"value":"0,0E+00","module":"A1-A3"},{"value":"0,0E+00","module":"C2"},{"value":"0,0E+00","module":"C3"},{"value":"0,0E+00","module":"C4"},{"value":"0,0E+00","module":"D"}]},{"parameter":"NRSF","unit":"MJ","values":[{"value":"0,0E+00","module":"A1-A3"},{"value":"0,0E+00","module":"C2"},{"value":"0,0E+00","module":"C3"},{"value":"0,0E+00","module":"C4"},{"value":"0,0E+00","module":"D"}]},{"parameter":"FW","unit":"m3","values":[{"value":"7,17E+00","module":"A1-A3"},{"value":"1,31E-02","module":"C2"},{"value":"3,52E-02","module":"C3"},{"value":"0,0E+00","module":"C4"},{"value":"-2,50E+00","module":"D"}]}],"end_of_life_waste":[{"parameter":"HWD","unit":"kg","values":[{"value":"6,97E-01","module":"A1-A3"},{"value":null,"module":"C2"},{"value":null,"module":"C3"},{"value":"0,0E+00","module":"C4"},{"value":null,"module":"D"}]},{"parameter":"NHWD","unit":"kg","values":[{"value":"0,0E+00","module":"A1-A3"},{"value":null,"module":"C2"},{"value":null,"module":"C3"},{"value":"0,0E+00","module":"C4"},{"value":null,"module":"D"}]},{"parameter":"RWD","unit":"kg","values":[{"value":"0,0E+00","module":"A1-A3"},{"value":null,"module":"C2"},{"value":null,"module":"C3"},{"value":"0,0E+00","module":"C4"},{"value":null,"module":"D"}]}],"end_of_life_flow":[{"parameter":"CRU","unit":"kg","values":[{"value":"0,0E+00","module":"A1-A3"},{"value":null,"module":"C2"},{"value":"0,0E+00","module":"C3"},{"value":"0,0E+00","module":"C4"},{"value":null,"module":"D"}]},{"parameter":"MFR","unit":"kg","values":[{"value":"3,82E+01","module":"A1-A3"},{"value":null,"module":"C2"},{"value":"1,00E+03","module":"C3"},{"value":"0,0E+00","module":"C4"},{"value":null,"module":"D"}]},{"parameter":"MER","unit":"kg","values":[{"value":"0,0E+00","module":"A1-A3"},{"value":null,"module":"C2"},{"value":"0,0E+00","module":"C3"},{"value":"0,0E+00","module":"C4"},{"value":null,"module":"D"}]},{"parameter":"EEE","unit":"MJ","values":[{"value":"0,0E+00","module":"A1-A3"},{"value":null,"module":"C2"},{"value":"0,0E+00","module":"C3"},{"value":"0,0E+00","module":"C4"},{"value":null,"module":"D"}]},{"parameter":"EET","unit":"MJ","values":[{"value":"0,0E+00","module":"A1-A3"},{"value":null,"module":"C2"},{"value":"0,0E+00","module":"C3"},{"value":"0,0E+00","module":"C4"},{"value":null,"module":"D"}]}]}