{"product_name":"Component EPD Surnadal: PVC insulated and PVC sheathed house wiring cable for open, fixed installation indoors and outdoors PR 2x1,5/1,5","epd_id":"NEPD-8141-7805","compliance":["EN 15804+A2","ISO 14025","ISO 21930"],"producer_name":"Pipelife Norge AS","environmental_impact":[{"parameter":"GWP-total","unit":"kg CO2-eq.","values":[{"value":"3,91E+00","module":"A1-A3"},{"value":"1,63E-02","module":"A4"},{"value":"0,0E+00","module":"C1"},{"value":"0,0E+00","module":"C2"},{"value":"0,0E+00","module":"C3"},{"value":"0,0E+00","module":"C4"},{"value":"0,0E+00","module":"D"}]},{"parameter":"GWP-fossil","unit":"kg CO2-eq.","values":[{"value":"3,88E+00","module":"A1-A3"},{"value":"1,63E-02","module":"A4"},{"value":"0,0E+00","module":"C1"},{"value":"0,0E+00","module":"C2"},{"value":"0,0E+00","module":"C3"},{"value":"0,0E+00","module":"C4"},{"value":"0,0E+00","module":"D"}]},{"parameter":"GWP-biogenic","unit":"kg CO2-eq.","values":[{"value":"2,10E-02","module":"A1-A3"},{"value":"6,76E-06","module":"A4"},{"value":"0,0E+00","module":"C1"},{"value":"0,0E+00","module":"C2"},{"value":"0,0E+00","module":"C3"},{"value":"0,0E+00","module":"C4"},{"value":"0,0E+00","module":"D"}]},{"parameter":"GWP-luluc","unit":"kg CO2-eq.","values":[{"value":"1,10E-02","module":"A1-A3"},{"value":"5,81E-06","module":"A4"},{"value":"0,0E+00","module":"C1"},{"value":"0,0E+00","module":"C2"},{"value":"0,0E+00","module":"C3"},{"value":"0,0E+00","module":"C4"},{"value":"0,0E+00","module":"D"}]},{"parameter":"ODP","unit":"kg CFC 11-eq.","values":[{"value":"3,71E-08","module":"A1-A3"},{"value":"3,70E-09","module":"A4"},{"value":"0,0E+00","module":"C1"},{"value":"0,0E+00","module":"C2"},{"value":"0,0E+00","module":"C3"},{"value":"0,0E+00","module":"C4"},{"value":"0,0E+00","module":"D"}]},{"parameter":"AP","unit":"mol H+-eq.","values":[{"value":"3,73E-02","module":"A1-A3"},{"value":"4,69E-05","module":"A4"},{"value":"0,0E+00","module":"C1"},{"value":"0,0E+00","module":"C2"},{"value":"0,0E+00","module":"C3"},{"value":"0,0E+00","module":"C4"},{"value":"0,0E+00","module":"D"}]},{"parameter":"POCP","unit":"kg NMVOC-eq.","values":[{"value":"1,11E-02","module":"A1-A3"},{"value":"3,98E-05","module":"A4"},{"value":"0,0E+00","module":"C1"},{"value":"0,0E+00","module":"C2"},{"value":"0,0E+00","module":"C3"},{"value":"0,0E+00","module":"C4"},{"value":"0,0E+00","module":"D"}]},{"parameter":"ADPE","unit":"kg Sb-eq.","values":[{"value":"1,40E-03","module":"A1-A3"},{"value":"4,51E-07","module":"A4"},{"value":"0,0E+00","module":"C1"},{"value":"0,0E+00","module":"C2"},{"value":"0,0E+00","module":"C3"},{"value":"0,0E+00","module":"C4"},{"value":"0,0E+00","module":"D"}]},{"parameter":"ADPF","unit":"MJ","values":[{"value":"6,48E+01","module":"A1-A3"},{"value":"2,47E-01","module":"A4"},{"value":"0,0E+00","module":"C1"},{"value":"0,0E+00","module":"C2"},{"value":"0,0E+00","module":"C3"},{"value":"0,0E+00","module":"C4"},{"value":"0,0E+00","module":"D"}]},{"parameter":"WDP","unit":"m3 world-eq.","values":[{"value":"3,51E+00","module":"A1-A3"},{"value":"2,39E-01","module":"A4"},{"value":"0,0E+00","module":"C1"},{"value":"0,0E+00","module":"C2"},{"value":"0,0E+00","module":"C3"},{"value":"0,0E+00","module":"C4"},{"value":"0,0E+00","module":"D"}]},{"parameter":"EP-freshwater","unit":"kg P-eq.","values":[{"value":"9,58E-06","module":"A1-A3"},{"value":"1,31E-07","module":"A4"},{"value":"0,0E+00","module":"C1"},{"value":"0,0E+00","module":"C2"},{"value":"0,0E+00","module":"C3"},{"value":"0,0E+00","module":"C4"},{"value":"0,0E+00","module":"D"}]},{"parameter":"EP-marine","unit":"kg N-eq.","values":[{"value":"2,95E-03","module":"A1-A3"},{"value":"9,29E-06","module":"A4"},{"value":"0,0E+00","module":"C1"},{"value":"0,0E+00","module":"C2"},{"value":"0,0E+00","module":"C3"},{"value":"0,0E+00","module":"C4"},{"value":"0,0E+00","module":"D"}]},{"parameter":"EP-terrestrial","unit":"mol N-eq.","values":[{"value":"3,11E-02","module":"A1-A3"},{"value":"1,04E-04","module":"A4"},{"value":"0,0E+00","module":"C1"},{"value":"0,0E+00","module":"C2"},{"value":"0,0E+00","module":"C3"},{"value":"0,0E+00","module":"C4"},{"value":"0,0E+00","module":"D"}]},{"parameter":"GWP-IOBC","unit":"kg CO2-eq.","values":[{"value":"3,83E+00","module":"A1-A3"},{"value":"1,63E-02","module":"A4"},{"value":"0,0E+00","module":"C1"},{"value":"0,0E+00","module":"C2"},{"value":"0,0E+00","module":"C3"},{"value":"0,0E+00","module":"C4"},{"value":"0,0E+00","module":"D"}]}],"additional_environmental_impact":[{"parameter":"PM","unit":"disease incidence","values":[{"value":"1,00E-08","module":"A1-A3"},{"value":"1,00E-09","module":"A4"},{"value":"0,0E+00","module":"C1"},{"value":"0,0E+00","module":"C2"},{"value":"0,0E+00","module":"C3"},{"value":"0,0E+00","module":"C4"},{"value":"0,0E+00","module":"D"}]},{"parameter":"ETP-fw","unit":"CTUe","values":[{"value":"1,83E+00","module":"A1-A3"},{"value":"1,83E-01","module":"A4"},{"value":"0,0E+00","module":"C1"},{"value":"0,0E+00","module":"C2"},{"value":"0,0E+00","module":"C3"},{"value":"0,0E+00","module":"C4"},{"value":"0,0E+00","module":"D"}]},{"parameter":"HTP-c","unit":"CTUh","values":[{"value":"0,0E+00","module":"A1-A3"},{"value":"0,0E+00","module":"A4"},{"value":"0,0E+00","module":"C1"},{"value":"0,0E+00","module":"C2"},{"value":"0,0E+00","module":"C3"},{"value":"0,0E+00","module":"C4"},{"value":"0,0E+00","module":"D"}]},{"parameter":"HTP-nc","unit":"CTUh","values":[{"value":"2,00E-09","module":"A1-A3"},{"value":"2,00E-10","module":"A4"},{"value":"0,0E+00","module":"C1"},{"value":"0,0E+00","module":"C2"},{"value":"0,0E+00","module":"C3"},{"value":"0,0E+00","module":"C4"},{"value":"0,0E+00","module":"D"}]},{"parameter":"SQP","unit":"unitless","values":[{"value":"1,73E+00","module":"A1-A3"},{"value":"1,73E-01","module":"A4"},{"value":"0,0E+00","module":"C1"},{"value":"0,0E+00","module":"C2"},{"value":"0,0E+00","module":"C3"},{"value":"0,0E+00","module":"C4"},{"value":"0,0E+00","module":"D"}]},{"parameter":"IRP","unit":"kBq U235-eq.","values":[{"value":"1,08E-02","module":"A1-A3"},{"value":"1,08E-03","module":"A4"},{"value":"0,0E+00","module":"C1"},{"value":"0,0E+00","module":"C2"},{"value":"0,0E+00","module":"C3"},{"value":"0,0E+00","module":"C4"},{"value":"0,0E+00","module":"D"}]}],"resource_use":[{"parameter":"PERE","unit":"MJ","values":[{"value":"1,14E+01","module":"A1-A3"},{"value":"3,54E-03","module":"A4"},{"value":"0,0E+00","module":"C1"},{"value":"0,0E+00","module":"C2"},{"value":"0,0E+00","module":"C3"},{"value":"0,0E+00","module":"C4"},{"value":"0,0E+00","module":"D"}]},{"parameter":"PERM","unit":"MJ","values":[{"value":"0,0E+00","module":"A1-A3"},{"value":"0,0E+00","module":"A4"},{"value":"0,0E+00","module":"C1"},{"value":"0,0E+00","module":"C2"},{"value":"0,0E+00","module":"C3"},{"value":"0,0E+00","module":"C4"},{"value":"0,0E+00","module":"D"}]},{"parameter":"PERT","unit":"MJ","values":[{"value":"1,14E+01","module":"A1-A3"},{"value":"3,54E-03","module":"A4"},{"value":"0,0E+00","module":"C1"},{"value":"0,0E+00","module":"C2"},{"value":"0,0E+00","module":"C3"},{"value":"0,0E+00","module":"C4"},{"value":"0,0E+00","module":"D"}]},{"parameter":"PENRE","unit":"MJ","values":[{"value":"5,30E+01","module":"A1-A3"},{"value":"2,47E-01","module":"A4"},{"value":"0,0E+00","module":"C1"},{"value":"0,0E+00","module":"C2"},{"value":"0,0E+00","module":"C3"},{"value":"0,0E+00","module":"C4"},{"value":"0,0E+00","module":"D"}]},{"parameter":"PENRM","unit":"MJ","values":[{"value":"1,15E+01","module":"A1-A3"},{"value":"0,0E+00","module":"A4"},{"value":"0,0E+00","module":"C1"},{"value":"0,0E+00","module":"C2"},{"value":"0,0E+00","module":"C3"},{"value":"0,0E+00","module":"C4"},{"value":"0,0E+00","module":"D"}]},{"parameter":"PENRT","unit":"MJ","values":[{"value":"6,45E+01","module":"A1-A3"},{"value":"2,47E-01","module":"A4"},{"value":"0,0E+00","module":"C1"},{"value":"0,0E+00","module":"C2"},{"value":"0,0E+00","module":"C3"},{"value":"0,0E+00","module":"C4"},{"value":"0,0E+00","module":"D"}]},{"parameter":"SM","unit":"kg","values":[{"value":"0,0E+00","module":"A1-A3"},{"value":"0,0E+00","module":"A4"},{"value":"0,0E+00","module":"C1"},{"value":"0,0E+00","module":"C2"},{"value":"0,0E+00","module":"C3"},{"value":"0,0E+00","module":"C4"},{"value":"0,0E+00","module":"D"}]},{"parameter":"RSF","unit":"MJ","values":[{"value":"1,27E-03","module":"A1-A3"},{"value":"1,26E-04","module":"A4"},{"value":"0,0E+00","module":"C1"},{"value":"0,0E+00","module":"C2"},{"value":"0,0E+00","module":"C3"},{"value":"0,0E+00","module":"C4"},{"value":"0,0E+00","module":"D"}]},{"parameter":"NRSF","unit":"MJ","values":[{"value":"4,53E-03","module":"A1-A3"},{"value":"4,52E-04","module":"A4"},{"value":"0,0E+00","module":"C1"},{"value":"0,0E+00","module":"C2"},{"value":"0,0E+00","module":"C3"},{"value":"0,0E+00","module":"C4"},{"value":"0,0E+00","module":"D"}]},{"parameter":"FW","unit":"m3","values":[{"value":"3,60E-02","module":"A1-A3"},{"value":"2,64E-05","module":"A4"},{"value":"0,0E+00","module":"C1"},{"value":"0,0E+00","module":"C2"},{"value":"0,0E+00","module":"C3"},{"value":"0,0E+00","module":"C4"},{"value":"0,0E+00","module":"D"}]}],"end_of_life_waste":[{"parameter":"HWD","unit":"kg","values":[{"value":"1,28E-04","module":"A1-A3"},{"value":"1,27E-05","module":"A4"},{"value":"0,0E+00","module":"C1"},{"value":"0,0E+00","module":"C2"},{"value":"0,0E+00","module":"C3"},{"value":"0,0E+00","module":"C4"},{"value":"0,0E+00","module":"D"}]},{"parameter":"NHWD","unit":"kg","values":[{"value":"1,41E-01","module":"A1-A3"},{"value":"1,20E-02","module":"A4"},{"value":"0,0E+00","module":"C1"},{"value":"0,0E+00","module":"C2"},{"value":"0,0E+00","module":"C3"},{"value":"0,0E+00","module":"C4"},{"value":"0,0E+00","module":"D"}]},{"parameter":"RWD","unit":"kg","values":[{"value":"1,69E-05","module":"A1-A3"},{"value":"1,68E-06","module":"A4"},{"value":"0,0E+00","module":"C1"},{"value":"0,0E+00","module":"C2"},{"value":"0,0E+00","module":"C3"},{"value":"0,0E+00","module":"C4"},{"value":"0,0E+00","module":"D"}]}],"end_of_life_flow":[{"parameter":"CRU","unit":"kg","values":[{"value":"0,0E+00","module":"A1-A3"},{"value":"0,0E+00","module":"A4"},{"value":"0,0E+00","module":"C1"},{"value":"0,0E+00","module":"C2"},{"value":"0,0E+00","module":"C3"},{"value":"0,0E+00","module":"C4"},{"value":"0,0E+00","module":"D"}]},{"parameter":"MFR","unit":"kg","values":[{"value":"0,0E+00","module":"A1-A3"},{"value":"0,0E+00","module":"A4"},{"value":"0,0E+00","module":"C1"},{"value":"0,0E+00","module":"C2"},{"value":"0,0E+00","module":"C3"},{"value":"0,0E+00","module":"C4"},{"value":"0,0E+00","module":"D"}]},{"parameter":"MER","unit":"kg","values":[{"value":"0,0E+00","module":"A1-A3"},{"value":"0,0E+00","module":"A4"},{"value":"0,0E+00","module":"C1"},{"value":"0,0E+00","module":"C2"},{"value":"0,0E+00","module":"C3"},{"value":"0,0E+00","module":"C4"},{"value":"0,0E+00","module":"D"}]},{"parameter":"EEE","unit":"MJ","values":[{"value":"0,0E+00","module":"A1-A3"},{"value":"0,0E+00","module":"A4"},{"value":"0,0E+00","module":"C1"},{"value":"0,0E+00","module":"C2"},{"value":"0,0E+00","module":"C3"},{"value":"0,0E+00","module":"C4"},{"value":"0,0E+00","module":"D"}]},{"parameter":"EET","unit":"MJ","values":[{"value":"0,0E+00","module":"A1-A3"},{"value":"0,0E+00","module":"A4"},{"value":"0,0E+00","module":"C1"},{"value":"0,0E+00","module":"C2"},{"value":"0,0E+00","module":"C3"},{"value":"0,0E+00","module":"C4"},{"value":"0,0E+00","module":"D"}]}]}