{
    "product_name": "Cold-formed welded structural hollow sections of non-alloy and fine grains steels ",
    "epd_id": "DAP 001:2023",
    "declared_unit": {
        "unit": "ton",
        "amount": 1.0
    },
    "compliance": [
        "EN 15804+A2",
        "ISO 14025"
    ],
    "producer_name": "Ferpinta \u2013 Ind\u00fastrias de Tubos de A\u00e7o de Fernando Pinho Teixeira, S.A.",
    "environmental_impact": [
        {
            "parameter": "GWP-total",
            "values": [
                {
                    "value": "2,50E+03",
                    "module": "A1-A3",
                    "scenario": null
                },
                {
                    "value": "4,15E+01",
                    "module": "C2",
                    "scenario": null
                },
                {
                    "value": "1,29E+01",
                    "module": "C3",
                    "scenario": null
                },
                {
                    "value": "0,00E+00",
                    "module": "C4",
                    "scenario": null
                },
                {
                    "value": "-1,43E+03",
                    "module": "D",
                    "scenario": null
                }
            ]
        },
        {
            "parameter": "GWP-fossil",
            "values": [
                {
                    "value": "2,47E+03",
                    "module": "A1-A3",
                    "scenario": null
                },
                {
                    "value": "4,14E+01",
                    "module": "C2",
                    "scenario": null
                },
                {
                    "value": "1,27E+01",
                    "module": "C3",
                    "scenario": null
                },
                {
                    "value": "0,00E+00",
                    "module": "C4",
                    "scenario": null
                },
                {
                    "value": "-1,41E+03",
                    "module": "D",
                    "scenario": null
                }
            ]
        },
        {
            "parameter": "GWP-biogenic",
            "values": [
                {
                    "value": "2,87E+01",
                    "module": "A1-A3",
                    "scenario": null
                },
                {
                    "value": "3,31E-02",
                    "module": "C2",
                    "scenario": null
                },
                {
                    "value": "1,32E-01",
                    "module": "C3",
                    "scenario": null
                },
                {
                    "value": "0,00E+00",
                    "module": "C4",
                    "scenario": null
                },
                {
                    "value": "-1,87E+01",
                    "module": "D",
                    "scenario": null
                }
            ]
        },
        {
            "parameter": "GWP-luluc",
            "values": [
                {
                    "value": "1,23E+00",
                    "module": "A1-A3",
                    "scenario": null
                },
                {
                    "value": "3,14E-04",
                    "module": "C2",
                    "scenario": null
                },
                {
                    "value": "1,72E-02",
                    "module": "C3",
                    "scenario": null
                },
                {
                    "value": "0,00E+00",
                    "module": "C4",
                    "scenario": null
                },
                {
                    "value": "4,39E-01",
                    "module": "D",
                    "scenario": null
                }
            ]
        },
        {
            "parameter": "ODP",
            "values": [
                {
                    "value": "1,22E-04",
                    "module": "A1-A3",
                    "scenario": null
                },
                {
                    "value": "9,61E-06",
                    "module": "C2",
                    "scenario": null
                },
                {
                    "value": "2,15E-06",
                    "module": "C3",
                    "scenario": null
                },
                {
                    "value": "0,00E+00",
                    "module": "C4",
                    "scenario": null
                },
                {
                    "value": "-5,06E-05",
                    "module": "D",
                    "scenario": null
                }
            ]
        },
        {
            "parameter": "AP",
            "values": [
                {
                    "value": "1,08E+01",
                    "module": "A1-A3",
                    "scenario": null
                },
                {
                    "value": "1,43E-01",
                    "module": "C2",
                    "scenario": null
                },
                {
                    "value": "1,19E-01",
                    "module": "C3",
                    "scenario": null
                },
                {
                    "value": "0,00E+00",
                    "module": "C4",
                    "scenario": null
                },
                {
                    "value": "-5,23E+00",
                    "module": "D",
                    "scenario": null
                }
            ]
        },
        {
            "parameter": "POCP",
            "values": [
                {
                    "value": "1,13E+01",
                    "module": "A1-A3",
                    "scenario": null
                },
                {
                    "value": "1,38E-01",
                    "module": "C2",
                    "scenario": null
                },
                {
                    "value": "1,36E-01",
                    "module": "C3",
                    "scenario": null
                },
                {
                    "value": "0,00E+00",
                    "module": "C4",
                    "scenario": null
                },
                {
                    "value": "-6,70E+00",
                    "module": "D",
                    "scenario": null
                }
            ]
        },
        {
            "parameter": "ADPE",
            "values": [
                {
                    "value": "2,65E-02",
                    "module": "A1-A3",
                    "scenario": null
                },
                {
                    "value": "1,76E-06",
                    "module": "C2",
                    "scenario": null
                },
                {
                    "value": "4,92E-07",
                    "module": "C3",
                    "scenario": null
                },
                {
                    "value": "0,00E+00",
                    "module": "C4",
                    "scenario": null
                },
                {
                    "value": "-2,40E-02",
                    "module": "D",
                    "scenario": null
                }
            ]
        },
        {
            "parameter": "ADPF",
            "values": [
                {
                    "value": "2,59E+04",
                    "module": "A1-A3",
                    "scenario": null
                },
                {
                    "value": "5,87E+02",
                    "module": "C2",
                    "scenario": null
                },
                {
                    "value": "1,98E+02",
                    "module": "C3",
                    "scenario": null
                },
                {
                    "value": "0,00E+00",
                    "module": "C4",
                    "scenario": null
                },
                {
                    "value": "-1,24E+04",
                    "module": "D",
                    "scenario": null
                }
            ]
        },
        {
            "parameter": "WDP",
            "values": [
                {
                    "value": "7,46E+02",
                    "module": "A1-A3",
                    "scenario": null
                },
                {
                    "value": "-1,24E-01",
                    "module": "C2",
                    "scenario": null
                },
                {
                    "value": "1,10E+00",
                    "module": "C3",
                    "scenario": null
                },
                {
                    "value": "0,00E+00",
                    "module": "C4",
                    "scenario": null
                },
                {
                    "value": "-6,48E+01",
                    "module": "D",
                    "scenario": null
                }
            ]
        },
        {
            "parameter": "EP-freshwater",
            "values": [
                {
                    "value": "1,13E-01",
                    "module": "A1-A3",
                    "scenario": null
                },
                {
                    "value": "2,26E-05",
                    "module": "C2",
                    "scenario": null
                },
                {
                    "value": "2,09E-04",
                    "module": "C3",
                    "scenario": null
                },
                {
                    "value": "0,00E+00",
                    "module": "C4",
                    "scenario": null
                },
                {
                    "value": "-6,99E-02",
                    "module": "D",
                    "scenario": null
                }
            ]
        },
        {
            "parameter": "EP-marine",
            "values": [
                {
                    "value": "2,26E+00",
                    "module": "A1-A3",
                    "scenario": null
                },
                {
                    "value": "4,60E-02",
                    "module": "C2",
                    "scenario": null
                },
                {
                    "value": "4,55E-02",
                    "module": "C3",
                    "scenario": null
                },
                {
                    "value": "0,00E+00",
                    "module": "C4",
                    "scenario": null
                },
                {
                    "value": "-1,10E+00",
                    "module": "D",
                    "scenario": null
                }
            ]
        },
        {
            "parameter": "EP-terrestrial",
            "values": [
                {
                    "value": "2,46E+01",
                    "module": "A1-A3",
                    "scenario": null
                },
                {
                    "value": "5,06E-01",
                    "module": "C2",
                    "scenario": null
                },
                {
                    "value": "5,00E-01",
                    "module": "C3",
                    "scenario": null
                },
                {
                    "value": "0,00E+00",
                    "module": "C4",
                    "scenario": null
                },
                {
                    "value": "-1,21E+01",
                    "module": "D",
                    "scenario": null
                }
            ]
        }
    ],
    "additional_environmental_impact": [
        {
            "parameter": "PM",
            "values": [
                {
                    "value": null,
                    "module": "A1-A3",
                    "scenario": null
                },
                {
                    "value": null,
                    "module": "C2",
                    "scenario": null
                },
                {
                    "value": null,
                    "module": "C3",
                    "scenario": null
                },
                {
                    "value": null,
                    "module": "C4",
                    "scenario": null
                },
                {
                    "value": null,
                    "module": "D",
                    "scenario": null
                }
            ]
        },
        {
            "parameter": "ETP-fw",
            "values": [
                {
                    "value": null,
                    "module": "A1-A3",
                    "scenario": null
                },
                {
                    "value": null,
                    "module": "C2",
                    "scenario": null
                },
                {
                    "value": null,
                    "module": "C3",
                    "scenario": null
                },
                {
                    "value": null,
                    "module": "C4",
                    "scenario": null
                },
                {
                    "value": null,
                    "module": "D",
                    "scenario": null
                }
            ]
        },
        {
            "parameter": "HTP-c",
            "values": [
                {
                    "value": null,
                    "module": "A1-A3",
                    "scenario": null
                },
                {
                    "value": null,
                    "module": "C2",
                    "scenario": null
                },
                {
                    "value": null,
                    "module": "C3",
                    "scenario": null
                },
                {
                    "value": null,
                    "module": "C4",
                    "scenario": null
                },
                {
                    "value": null,
                    "module": "D",
                    "scenario": null
                }
            ]
        },
        {
            "parameter": "HTP-nc",
            "values": [
                {
                    "value": null,
                    "module": "A1-A3",
                    "scenario": null
                },
                {
                    "value": null,
                    "module": "C2",
                    "scenario": null
                },
                {
                    "value": null,
                    "module": "C3",
                    "scenario": null
                },
                {
                    "value": null,
                    "module": "C4",
                    "scenario": null
                },
                {
                    "value": null,
                    "module": "D",
                    "scenario": null
                }
            ]
        },
        {
            "parameter": "SQP",
            "values": [
                {
                    "value": null,
                    "module": "A1-A3",
                    "scenario": null
                },
                {
                    "value": null,
                    "module": "C2",
                    "scenario": null
                },
                {
                    "value": null,
                    "module": "C3",
                    "scenario": null
                },
                {
                    "value": null,
                    "module": "C4",
                    "scenario": null
                },
                {
                    "value": null,
                    "module": "D",
                    "scenario": null
                }
            ]
        },
        {
            "parameter": "IRP",
            "values": [
                {
                    "value": null,
                    "module": "A1-A3",
                    "scenario": null
                },
                {
                    "value": null,
                    "module": "C2",
                    "scenario": null
                },
                {
                    "value": null,
                    "module": "C3",
                    "scenario": null
                },
                {
                    "value": null,
                    "module": "C4",
                    "scenario": null
                },
                {
                    "value": null,
                    "module": "D",
                    "scenario": null
                }
            ]
        }
    ],
    "resource_use": [
        {
            "parameter": "PERE",
            "values": [
                {
                    "value": "2,24E+03",
                    "module": "A1-A3",
                    "scenario": null
                },
                {
                    "value": "8,63E-01",
                    "module": "C2",
                    "scenario": null
                },
                {
                    "value": "1,35E+01",
                    "module": "C3",
                    "scenario": null
                },
                {
                    "value": "0,00E+00",
                    "module": "C4",
                    "scenario": null
                },
                {
                    "value": "-8,95E+00",
                    "module": "D",
                    "scenario": null
                }
            ]
        },
        {
            "parameter": "PERM",
            "values": [
                {
                    "value": "6,22E+01",
                    "module": "A1-A3",
                    "scenario": null
                },
                {
                    "value": "0,00E+00",
                    "module": "C2",
                    "scenario": null
                },
                {
                    "value": "0,00E+00",
                    "module": "C3",
                    "scenario": null
                },
                {
                    "value": "0,00E+00",
                    "module": "C4",
                    "scenario": null
                },
                {
                    "value": "0,00E+00",
                    "module": "D",
                    "scenario": null
                }
            ]
        },
        {
            "parameter": "PERT",
            "values": [
                {
                    "value": "2,31E+03",
                    "module": "A1-A3",
                    "scenario": null
                },
                {
                    "value": "8,63E-01",
                    "module": "C2",
                    "scenario": null
                },
                {
                    "value": "1,35E+01",
                    "module": "C3",
                    "scenario": null
                },
                {
                    "value": "0,00E+00",
                    "module": "C4",
                    "scenario": null
                },
                {
                    "value": "-8,95E+02",
                    "module": "D",
                    "scenario": null
                }
            ]
        },
        {
            "parameter": "PENRE",
            "values": [
                {
                    "value": "2,59E+04",
                    "module": "A1-A3",
                    "scenario": null
                },
                {
                    "value": "5,87E+02",
                    "module": "C2",
                    "scenario": null
                },
                {
                    "value": "1,98E+02",
                    "module": "C3",
                    "scenario": null
                },
                {
                    "value": "0,00E+00",
                    "module": "C4",
                    "scenario": null
                },
                {
                    "value": "-1,24E+04",
                    "module": "D",
                    "scenario": null
                }
            ]
        },
        {
            "parameter": "PENRM",
            "values": [
                {
                    "value": "5,09E+01",
                    "module": "A1-A3",
                    "scenario": null
                },
                {
                    "value": "0,00E+00",
                    "module": "C2",
                    "scenario": null
                },
                {
                    "value": "0,00E+00",
                    "module": "C3",
                    "scenario": null
                },
                {
                    "value": "0,00E+00",
                    "module": "C4",
                    "scenario": null
                },
                {
                    "value": "0,00E+00",
                    "module": "D",
                    "scenario": null
                }
            ]
        },
        {
            "parameter": "PENRT",
            "values": [
                {
                    "value": "2,59E+04",
                    "module": "A1-A3",
                    "scenario": null
                },
                {
                    "value": "5,87E+02",
                    "module": "C2",
                    "scenario": null
                },
                {
                    "value": "1,98E+02",
                    "module": "C3",
                    "scenario": null
                },
                {
                    "value": "0,00E+00",
                    "module": "C4",
                    "scenario": null
                },
                {
                    "value": "-1,24E+04",
                    "module": "D",
                    "scenario": null
                }
            ]
        },
        {
            "parameter": "SM",
            "values": [
                {
                    "value": "2,19E+01",
                    "module": "A1-A3",
                    "scenario": null
                },
                {
                    "value": "0,00E+00",
                    "module": "C2",
                    "scenario": null
                },
                {
                    "value": "0,00E+00",
                    "module": "C3",
                    "scenario": null
                },
                {
                    "value": "0,00E+00",
                    "module": "C4",
                    "scenario": null
                },
                {
                    "value": "0,00E+00",
                    "module": "D",
                    "scenario": null
                }
            ]
        },
        {
            "parameter": "RSF",
            "values": [
                {
                    "value": "0,00E+00",
                    "module": "A1-A3",
                    "scenario": null
                },
                {
                    "value": "0,00E+00",
                    "module": "C2",
                    "scenario": null
                },
                {
                    "value": "0,00E+00",
                    "module": "C3",
                    "scenario": null
                },
                {
                    "value": "0,00E+00",
                    "module": "C4",
                    "scenario": null
                },
                {
                    "value": "0,00E+00",
                    "module": "D",
                    "scenario": null
                }
            ]
        },
        {
            "parameter": "NRSF",
            "values": [
                {
                    "value": "0,00E+00",
                    "module": "A1-A3",
                    "scenario": null
                },
                {
                    "value": "0,00E+00",
                    "module": "C2",
                    "scenario": null
                },
                {
                    "value": "0,00E+00",
                    "module": "C3",
                    "scenario": null
                },
                {
                    "value": "0,00E+00",
                    "module": "C4",
                    "scenario": null
                },
                {
                    "value": "0,00E+00",
                    "module": "D",
                    "scenario": null
                }
            ]
        },
        {
            "parameter": "FW",
            "values": [
                {
                    "value": "1,34E+01",
                    "module": "A1-A3",
                    "scenario": null
                },
                {
                    "value": "8,81E-04",
                    "module": "C2",
                    "scenario": null
                },
                {
                    "value": "2,90E-02",
                    "module": "C3",
                    "scenario": null
                },
                {
                    "value": "0,00E+00",
                    "module": "C4",
                    "scenario": null
                },
                {
                    "value": "-5,77E+00",
                    "module": "D",
                    "scenario": null
                }
            ]
        }
    ],
    "end_of_life_waste": [
        {
            "parameter": "HWD",
            "values": [
                {
                    "value": "8,83E-01",
                    "module": "A1-A3",
                    "scenario": null
                },
                {
                    "value": null,
                    "module": "C2",
                    "scenario": null
                },
                {
                    "value": null,
                    "module": "C3",
                    "scenario": null
                },
                {
                    "value": "0,00E+00",
                    "module": "C4",
                    "scenario": null
                },
                {
                    "value": null,
                    "module": "D",
                    "scenario": null
                }
            ]
        },
        {
            "parameter": "NHWD",
            "values": [
                {
                    "value": "0,00E+00",
                    "module": "A1-A3",
                    "scenario": null
                },
                {
                    "value": null,
                    "module": "C2",
                    "scenario": null
                },
                {
                    "value": null,
                    "module": "C3",
                    "scenario": null
                },
                {
                    "value": "0,00E+00",
                    "module": "C4",
                    "scenario": null
                },
                {
                    "value": null,
                    "module": "D",
                    "scenario": null
                }
            ]
        },
        {
            "parameter": "RWD",
            "values": [
                {
                    "value": "0,00E+00",
                    "module": "A1-A3",
                    "scenario": null
                },
                {
                    "value": null,
                    "module": "C2",
                    "scenario": null
                },
                {
                    "value": null,
                    "module": "C3",
                    "scenario": null
                },
                {
                    "value": "0,00E+00",
                    "module": "C4",
                    "scenario": null
                },
                {
                    "value": null,
                    "module": "D",
                    "scenario": null
                }
            ]
        }
    ],
    "end_of_life_flow": [
        {
            "parameter": "CRU",
            "values": [
                {
                    "value": "0,00E+00",
                    "module": "A1-A3",
                    "scenario": null
                },
                {
                    "value": "0,00E+00",
                    "module": "C2",
                    "scenario": null
                },
                {
                    "value": "0,00E+00",
                    "module": "C3",
                    "scenario": null
                },
                {
                    "value": "0,00E+00",
                    "module": "C4",
                    "scenario": null
                },
                {
                    "value": "0,00E+00",
                    "module": "D",
                    "scenario": null
                }
            ]
        },
        {
            "parameter": "MFR",
            "values": [
                {
                    "value": "4,43E+01",
                    "module": "A1-A3",
                    "scenario": null
                },
                {
                    "value": "0,00E+00",
                    "module": "C2",
                    "scenario": null
                },
                {
                    "value": "1,00E+03",
                    "module": "C3",
                    "scenario": null
                },
                {
                    "value": "0,00E+00",
                    "module": "C4",
                    "scenario": null
                },
                {
                    "value": "0,00E+00",
                    "module": "D",
                    "scenario": null
                }
            ]
        },
        {
            "parameter": "MER",
            "values": [
                {
                    "value": "0,00E+00",
                    "module": "A1-A3",
                    "scenario": null
                },
                {
                    "value": "0,00E+00",
                    "module": "C2",
                    "scenario": null
                },
                {
                    "value": "0,00E+00",
                    "module": "C3",
                    "scenario": null
                },
                {
                    "value": "0,00E+00",
                    "module": "C4",
                    "scenario": null
                },
                {
                    "value": "0,00E+00",
                    "module": "D",
                    "scenario": null
                }
            ]
        },
        {
            "parameter": "EEE",
            "values": [
                {
                    "value": "0,00E+00",
                    "module": "A1-A3",
                    "scenario": null
                },
                {
                    "value": "0,00E+00",
                    "module": "C2",
                    "scenario": null
                },
                {
                    "value": "0,00E+00",
                    "module": "C3",
                    "scenario": null
                },
                {
                    "value": "0,00E+00",
                    "module": "C4",
                    "scenario": null
                },
                {
                    "value": "0,00E+00",
                    "module": "D",
                    "scenario": null
                }
            ]
        },
        {
            "parameter": "EET",
            "values": [
                {
                    "value": "0,00E+00",
                    "module": "A1-A3",
                    "scenario": null
                },
                {
                    "value": "0,00E+00",
                    "module": "C2",
                    "scenario": null
                },
                {
                    "value": "0,00E+00",
                    "module": "C3",
                    "scenario": null
                },
                {
                    "value": "0,00E+00",
                    "module": "C4",
                    "scenario": null
                },
                {
                    "value": "0,00E+00",
                    "module": "D",
                    "scenario": null
                }
            ]
        }
    ]
}