{"product_name":"Cold-formed welded structural hollow sections of non-alloy and fine grains steels ","epd_id":"DAP 001:2023","declared_unit":{"unit":"ton","amount":1},"compliance":["EN 15804+A2","ISO 14025"],"producer_name":"Ferpinta \u2013 Ind\u00fastrias de Tubos de A\u00e7o de Fernando Pinho Teixeira, S.A.","environmental_impact":[{"parameter":"GWP-total","unit":"kg CO2-eq","values":[{"value":"2,50E+03","module":"A1-A3","scenario":null},{"value":"4,15E+01","module":"C2","scenario":null},{"value":"1,29E+01","module":"C3","scenario":null},{"value":"0,00E+00","module":"C4","scenario":null},{"value":"-1,43E+03","module":"D","scenario":null}]},{"parameter":"GWP-fossil","unit":"kg CO2-eq","values":[{"value":"2,47E+03","module":"A1-A3","scenario":null},{"value":"4,14E+01","module":"C2","scenario":null},{"value":"1,27E+01","module":"C3","scenario":null},{"value":"0,00E+00","module":"C4","scenario":null},{"value":"-1,41E+03","module":"D","scenario":null}]},{"parameter":"GWP-biogenic","unit":"kg CO2-eq","values":[{"value":"2,87E+01","module":"A1-A3","scenario":null},{"value":"3,31E-02","module":"C2","scenario":null},{"value":"1,32E-01","module":"C3","scenario":null},{"value":"0,00E+00","module":"C4","scenario":null},{"value":"-1,87E+01","module":"D","scenario":null}]},{"parameter":"GWP-luluc","unit":"kg CO2-eq","values":[{"value":"1,23E+00","module":"A1-A3","scenario":null},{"value":"3,14E-04","module":"C2","scenario":null},{"value":"1,72E-02","module":"C3","scenario":null},{"value":"0,00E+00","module":"C4","scenario":null},{"value":"4,39E-01","module":"D","scenario":null}]},{"parameter":"ODP","unit":"kg CFC11-eq","values":[{"value":"1,22E-04","module":"A1-A3","scenario":null},{"value":"9,61E-06","module":"C2","scenario":null},{"value":"2,15E-06","module":"C3","scenario":null},{"value":"0,00E+00","module":"C4","scenario":null},{"value":"-5,06E-05","module":"D","scenario":null}]},{"parameter":"AP","unit":"mol H+-eq","values":[{"value":"1,08E+01","module":"A1-A3","scenario":null},{"value":"1,43E-01","module":"C2","scenario":null},{"value":"1,19E-01","module":"C3","scenario":null},{"value":"0,00E+00","module":"C4","scenario":null},{"value":"-5,23E+00","module":"D","scenario":null}]},{"parameter":"POCP","unit":"kg NMVOC-eq","values":[{"value":"1,13E+01","module":"A1-A3","scenario":null},{"value":"1,38E-01","module":"C2","scenario":null},{"value":"1,36E-01","module":"C3","scenario":null},{"value":"0,00E+00","module":"C4","scenario":null},{"value":"-6,70E+00","module":"D","scenario":null}]},{"parameter":"ADPE","unit":"kg Sb-eq","values":[{"value":"2,65E-02","module":"A1-A3","scenario":null},{"value":"1,76E-06","module":"C2","scenario":null},{"value":"4,92E-07","module":"C3","scenario":null},{"value":"0,00E+00","module":"C4","scenario":null},{"value":"-2,40E-02","module":"D","scenario":null}]},{"parameter":"ADPF","unit":"MJ","values":[{"value":"2,59E+04","module":"A1-A3","scenario":null},{"value":"5,87E+02","module":"C2","scenario":null},{"value":"1,98E+02","module":"C3","scenario":null},{"value":"0,00E+00","module":"C4","scenario":null},{"value":"-1,24E+04","module":"D","scenario":null}]},{"parameter":"WDP","unit":"m3 world-eq. Deprived","values":[{"value":"7,46E+02","module":"A1-A3","scenario":null},{"value":"-1,24E-01","module":"C2","scenario":null},{"value":"1,10E+00","module":"C3","scenario":null},{"value":"0,00E+00","module":"C4","scenario":null},{"value":"-6,48E+01","module":"D","scenario":null}]},{"parameter":"EP-freshwater","unit":"kg P-eq","values":[{"value":"1,13E-01","module":"A1-A3","scenario":null},{"value":"2,26E-05","module":"C2","scenario":null},{"value":"2,09E-04","module":"C3","scenario":null},{"value":"0,00E+00","module":"C4","scenario":null},{"value":"-6,99E-02","module":"D","scenario":null}]},{"parameter":"EP-marine","unit":"kg N-eq","values":[{"value":"2,26E+00","module":"A1-A3","scenario":null},{"value":"4,60E-02","module":"C2","scenario":null},{"value":"4,55E-02","module":"C3","scenario":null},{"value":"0,00E+00","module":"C4","scenario":null},{"value":"-1,10E+00","module":"D","scenario":null}]},{"parameter":"EP-terrestrial","unit":"mol N-eq.","values":[{"value":"2,46E+01","module":"A1-A3","scenario":null},{"value":"5,06E-01","module":"C2","scenario":null},{"value":"5,00E-01","module":"C3","scenario":null},{"value":"0,00E+00","module":"C4","scenario":null},{"value":"-1,21E+01","module":"D","scenario":null}]}],"additional_environmental_impact":[{"parameter":"PM","unit":"Disease incidence","values":[{"value":null,"module":"A1-A3","scenario":null},{"value":null,"module":"C2","scenario":null},{"value":null,"module":"C3","scenario":null},{"value":null,"module":"C4","scenario":null},{"value":null,"module":"D","scenario":null}]},{"parameter":"ETP-fw","unit":"CTUe","values":[{"value":null,"module":"A1-A3","scenario":null},{"value":null,"module":"C2","scenario":null},{"value":null,"module":"C3","scenario":null},{"value":null,"module":"C4","scenario":null},{"value":null,"module":"D","scenario":null}]},{"parameter":"HTP-c","unit":"CTUh","values":[{"value":null,"module":"A1-A3","scenario":null},{"value":null,"module":"C2","scenario":null},{"value":null,"module":"C3","scenario":null},{"value":null,"module":"C4","scenario":null},{"value":null,"module":"D","scenario":null}]},{"parameter":"HTP-nc","unit":"CTUh","values":[{"value":null,"module":"A1-A3","scenario":null},{"value":null,"module":"C2","scenario":null},{"value":null,"module":"C3","scenario":null},{"value":null,"module":"C4","scenario":null},{"value":null,"module":"D","scenario":null}]},{"parameter":"SQP","unit":"-","values":[{"value":null,"module":"A1-A3","scenario":null},{"value":null,"module":"C2","scenario":null},{"value":null,"module":"C3","scenario":null},{"value":null,"module":"C4","scenario":null},{"value":null,"module":"D","scenario":null}]},{"parameter":"IRP","unit":"kBq U235-eq","values":[{"value":null,"module":"A1-A3","scenario":null},{"value":null,"module":"C2","scenario":null},{"value":null,"module":"C3","scenario":null},{"value":null,"module":"C4","scenario":null},{"value":null,"module":"D","scenario":null}]}],"resource_use":[{"parameter":"PERE","unit":"MJ","values":[{"value":"2,24E+03","module":"A1-A3","scenario":null},{"value":"8,63E-01","module":"C2","scenario":null},{"value":"1,35E+01","module":"C3","scenario":null},{"value":"0,00E+00","module":"C4","scenario":null},{"value":"-8,95E+00","module":"D","scenario":null}]},{"parameter":"PERM","unit":"","values":[{"value":"6,22E+01","module":"A1-A3","scenario":null},{"value":"0,00E+00","module":"C2","scenario":null},{"value":"0,00E+00","module":"C3","scenario":null},{"value":"0,00E+00","module":"C4","scenario":null},{"value":"0,00E+00","module":"D","scenario":null}]},{"parameter":"PERT","unit":"MJ","values":[{"value":"2,31E+03","module":"A1-A3","scenario":null},{"value":"8,63E-01","module":"C2","scenario":null},{"value":"1,35E+01","module":"C3","scenario":null},{"value":"0,00E+00","module":"C4","scenario":null},{"value":"-8,95E+02","module":"D","scenario":null}]},{"parameter":"PENRE","unit":"MJ","values":[{"value":"2,59E+04","module":"A1-A3","scenario":null},{"value":"5,87E+02","module":"C2","scenario":null},{"value":"1,98E+02","module":"C3","scenario":null},{"value":"0,00E+00","module":"C4","scenario":null},{"value":"-1,24E+04","module":"D","scenario":null}]},{"parameter":"PENRM","unit":"MJ","values":[{"value":"5,09E+01","module":"A1-A3","scenario":null},{"value":"0,00E+00","module":"C2","scenario":null},{"value":"0,00E+00","module":"C3","scenario":null},{"value":"0,00E+00","module":"C4","scenario":null},{"value":"0,00E+00","module":"D","scenario":null}]},{"parameter":"PENRT","unit":"MJ","values":[{"value":"2,59E+04","module":"A1-A3","scenario":null},{"value":"5,87E+02","module":"C2","scenario":null},{"value":"1,98E+02","module":"C3","scenario":null},{"value":"0,00E+00","module":"C4","scenario":null},{"value":"-1,24E+04","module":"D","scenario":null}]},{"parameter":"SM","unit":"kg","values":[{"value":"2,19E+01","module":"A1-A3","scenario":null},{"value":"0,00E+00","module":"C2","scenario":null},{"value":"0,00E+00","module":"C3","scenario":null},{"value":"0,00E+00","module":"C4","scenario":null},{"value":"0,00E+00","module":"D","scenario":null}]},{"parameter":"RSF","unit":"MJ","values":[{"value":"0,00E+00","module":"A1-A3","scenario":null},{"value":"0,00E+00","module":"C2","scenario":null},{"value":"0,00E+00","module":"C3","scenario":null},{"value":"0,00E+00","module":"C4","scenario":null},{"value":"0,00E+00","module":"D","scenario":null}]},{"parameter":"NRSF","unit":"MJ","values":[{"value":"0,00E+00","module":"A1-A3","scenario":null},{"value":"0,00E+00","module":"C2","scenario":null},{"value":"0,00E+00","module":"C3","scenario":null},{"value":"0,00E+00","module":"C4","scenario":null},{"value":"0,00E+00","module":"D","scenario":null}]},{"parameter":"FW","unit":"m3","values":[{"value":"1,34E+01","module":"A1-A3","scenario":null},{"value":"8,81E-04","module":"C2","scenario":null},{"value":"2,90E-02","module":"C3","scenario":null},{"value":"0,00E+00","module":"C4","scenario":null},{"value":"-5,77E+00","module":"D","scenario":null}]}],"end_of_life_waste":[{"parameter":"HWD","unit":"kg","values":[{"value":"8,83E-01","module":"A1-A3","scenario":null},{"value":null,"module":"C2","scenario":null},{"value":null,"module":"C3","scenario":null},{"value":"0,00E+00","module":"C4","scenario":null},{"value":null,"module":"D","scenario":null}]},{"parameter":"NHWD","unit":"kg","values":[{"value":"0,00E+00","module":"A1-A3","scenario":null},{"value":null,"module":"C2","scenario":null},{"value":null,"module":"C3","scenario":null},{"value":"0,00E+00","module":"C4","scenario":null},{"value":null,"module":"D","scenario":null}]},{"parameter":"RWD","unit":"kg","values":[{"value":"0,00E+00","module":"A1-A3","scenario":null},{"value":null,"module":"C2","scenario":null},{"value":null,"module":"C3","scenario":null},{"value":"0,00E+00","module":"C4","scenario":null},{"value":null,"module":"D","scenario":null}]}],"end_of_life_flow":[{"parameter":"CRU","unit":"kg","values":[{"value":"0,00E+00","module":"A1-A3","scenario":null},{"value":"0,00E+00","module":"C2","scenario":null},{"value":"0,00E+00","module":"C3","scenario":null},{"value":"0,00E+00","module":"C4","scenario":null},{"value":"0,00E+00","module":"D","scenario":null}]},{"parameter":"MFR","unit":"kg","values":[{"value":"4,43E+01","module":"A1-A3","scenario":null},{"value":"0,00E+00","module":"C2","scenario":null},{"value":"1,00E+03","module":"C3","scenario":null},{"value":"0,00E+00","module":"C4","scenario":null},{"value":"0,00E+00","module":"D","scenario":null}]},{"parameter":"MER","unit":"kg","values":[{"value":"0,00E+00","module":"A1-A3","scenario":null},{"value":"0,00E+00","module":"C2","scenario":null},{"value":"0,00E+00","module":"C3","scenario":null},{"value":"0,00E+00","module":"C4","scenario":null},{"value":"0,00E+00","module":"D","scenario":null}]},{"parameter":"EEE","unit":"MJ","values":[{"value":"0,00E+00","module":"A1-A3","scenario":null},{"value":"0,00E+00","module":"C2","scenario":null},{"value":"0,00E+00","module":"C3","scenario":null},{"value":"0,00E+00","module":"C4","scenario":null},{"value":"0,00E+00","module":"D","scenario":null}]},{"parameter":"EET","unit":"MJ","values":[{"value":"0,00E+00","module":"A1-A3","scenario":null},{"value":"0,00E+00","module":"C2","scenario":null},{"value":"0,00E+00","module":"C3","scenario":null},{"value":"0,00E+00","module":"C4","scenario":null},{"value":"0,00E+00","module":"D","scenario":null}]}]}