{
    "product_name": "Cold-formed welded structural hollow sections of non-alloy and fine grains steels ",
    "epd_id": "DAP012:2024",
    "declared_unit": {
        "unit": "ton",
        "amount": 1.0
    },
    "compliance": [
        "EN 15804+A2",
        "ISO 14025"
    ],
    "producer_name": "Ferpinta \u2013 Ind\u00fastrias de Tubos de A\u00e7o de Fernando Pinho Teixeira, S.A.",
    "environmental_impact": [
        {
            "parameter": "GWP-total",
            "values": [
                {
                    "value": "1,81E+03",
                    "module": "A1-A3",
                    "scenario": null
                },
                {
                    "value": "2,44E+01",
                    "module": "C2",
                    "scenario": null
                },
                {
                    "value": "1,26E+01",
                    "module": "C3",
                    "scenario": null
                },
                {
                    "value": "0,00E+00",
                    "module": "C4",
                    "scenario": null
                },
                {
                    "value": "-8,70E+02",
                    "module": "D",
                    "scenario": null
                }
            ]
        },
        {
            "parameter": "GWP-fossil",
            "values": [
                {
                    "value": "1,80E+03",
                    "module": "A1-A3",
                    "scenario": null
                },
                {
                    "value": "2,44E+01",
                    "module": "C2",
                    "scenario": null
                },
                {
                    "value": "1,24E+01",
                    "module": "C3",
                    "scenario": null
                },
                {
                    "value": "0,00E+00",
                    "module": "C4",
                    "scenario": null
                },
                {
                    "value": "-8,60E+02",
                    "module": "D",
                    "scenario": null
                }
            ]
        },
        {
            "parameter": "GWP-biogenic",
            "values": [
                {
                    "value": "1,42E+01",
                    "module": "A1-A3",
                    "scenario": null
                },
                {
                    "value": "1,34E-02",
                    "module": "C2",
                    "scenario": null
                },
                {
                    "value": "1,66E-01",
                    "module": "C3",
                    "scenario": null
                },
                {
                    "value": "0,00E+00",
                    "module": "C4",
                    "scenario": null
                },
                {
                    "value": "-1,12E+01",
                    "module": "D",
                    "scenario": null
                }
            ]
        },
        {
            "parameter": "GWP-luluc",
            "values": [
                {
                    "value": "1,10E+00",
                    "module": "A1-A3",
                    "scenario": null
                },
                {
                    "value": "4,65E-04",
                    "module": "C2",
                    "scenario": null
                },
                {
                    "value": "2,04E-02",
                    "module": "C3",
                    "scenario": null
                },
                {
                    "value": "0,00E+00",
                    "module": "C4",
                    "scenario": null
                },
                {
                    "value": "2,90E-01",
                    "module": "D",
                    "scenario": null
                }
            ]
        },
        {
            "parameter": "ODP",
            "values": [
                {
                    "value": "3,42E-05",
                    "module": "A1-A3",
                    "scenario": null
                },
                {
                    "value": "5,04E-07",
                    "module": "C2",
                    "scenario": null
                },
                {
                    "value": "2,09E-07",
                    "module": "C3",
                    "scenario": null
                },
                {
                    "value": "0,00E+00",
                    "module": "C4",
                    "scenario": null
                },
                {
                    "value": "-1,70E-05",
                    "module": "D",
                    "scenario": null
                }
            ]
        },
        {
            "parameter": "AP",
            "values": [
                {
                    "value": "9,93E+00",
                    "module": "A1-A3",
                    "scenario": null
                },
                {
                    "value": "5,99E-02",
                    "module": "C2",
                    "scenario": null
                },
                {
                    "value": "1,02E-01",
                    "module": "C3",
                    "scenario": null
                },
                {
                    "value": "0,00E+00",
                    "module": "C4",
                    "scenario": null
                },
                {
                    "value": "-3,40E+00",
                    "module": "D",
                    "scenario": null
                }
            ]
        },
        {
            "parameter": "POCP",
            "values": [
                {
                    "value": "9,79E+00",
                    "module": "A1-A3",
                    "scenario": null
                },
                {
                    "value": "9,67E-02",
                    "module": "C2",
                    "scenario": null
                },
                {
                    "value": "1,42E-01",
                    "module": "C3",
                    "scenario": null
                },
                {
                    "value": "0,00E+00",
                    "module": "C4",
                    "scenario": null
                },
                {
                    "value": "-4,24E+00",
                    "module": "D",
                    "scenario": null
                }
            ]
        },
        {
            "parameter": "ADPE",
            "values": [
                {
                    "value": "6,11E-03",
                    "module": "A1-A3",
                    "scenario": null
                },
                {
                    "value": "8,15E-07",
                    "module": "C2",
                    "scenario": null
                },
                {
                    "value": "5,36E-07",
                    "module": "C3",
                    "scenario": null
                },
                {
                    "value": "0,00E+00",
                    "module": "C4",
                    "scenario": null
                },
                {
                    "value": "-7,66E-03",
                    "module": "D",
                    "scenario": null
                }
            ]
        },
        {
            "parameter": "ADPF",
            "values": [
                {
                    "value": "2,00E+04",
                    "module": "A1-A3",
                    "scenario": null
                },
                {
                    "value": "3,12E+02",
                    "module": "C2",
                    "scenario": null
                },
                {
                    "value": "1,93E+02",
                    "module": "C3",
                    "scenario": null
                },
                {
                    "value": "0,00E+00",
                    "module": "C4",
                    "scenario": null
                },
                {
                    "value": "-7,51E+03",
                    "module": "D",
                    "scenario": null
                }
            ]
        },
        {
            "parameter": "WDP",
            "values": [
                {
                    "value": "1,05E+02",
                    "module": "A1-A3",
                    "scenario": null
                },
                {
                    "value": "2,89E-01",
                    "module": "C2",
                    "scenario": null
                },
                {
                    "value": "1,33E+00",
                    "module": "C3",
                    "scenario": null
                },
                {
                    "value": "0,00E+00",
                    "module": "C4",
                    "scenario": null
                },
                {
                    "value": "-8,03E+01",
                    "module": "D",
                    "scenario": null
                }
            ]
        },
        {
            "parameter": "EP-freshwater",
            "values": [
                {
                    "value": "1,09E-01",
                    "module": "A1-A3",
                    "scenario": null
                },
                {
                    "value": "1,90E-05",
                    "module": "C2",
                    "scenario": null
                },
                {
                    "value": "1,16E-04",
                    "module": "C3",
                    "scenario": null
                },
                {
                    "value": "0,00E+00",
                    "module": "C4",
                    "scenario": null
                },
                {
                    "value": "-4,07E-02",
                    "module": "D",
                    "scenario": null
                }
            ]
        },
        {
            "parameter": "EP-marine",
            "values": [
                {
                    "value": "2,05E+00",
                    "module": "A1-A3",
                    "scenario": null
                },
                {
                    "value": "2,33E-02",
                    "module": "C2",
                    "scenario": null
                },
                {
                    "value": "4,41E-02",
                    "module": "C3",
                    "scenario": null
                },
                {
                    "value": "0,00E+00",
                    "module": "C4",
                    "scenario": null
                },
                {
                    "value": "-6,87E-01",
                    "module": "D",
                    "scenario": null
                }
            ]
        },
        {
            "parameter": "EP-terrestrial",
            "values": [
                {
                    "value": "2,23E+01",
                    "module": "A1-A3",
                    "scenario": null
                },
                {
                    "value": "2,45E-01",
                    "module": "C2",
                    "scenario": null
                },
                {
                    "value": "4,80E-01",
                    "module": "C3",
                    "scenario": null
                },
                {
                    "value": "0,00E+00",
                    "module": "C4",
                    "scenario": null
                },
                {
                    "value": "-7,96E+00",
                    "module": "D",
                    "scenario": null
                }
            ]
        }
    ],
    "additional_environmental_impact": [
        {
            "parameter": "PM",
            "values": [
                {
                    "value": null,
                    "module": "A1-A3",
                    "scenario": null
                },
                {
                    "value": null,
                    "module": "C2",
                    "scenario": null
                },
                {
                    "value": null,
                    "module": "C3",
                    "scenario": null
                },
                {
                    "value": null,
                    "module": "C4",
                    "scenario": null
                },
                {
                    "value": null,
                    "module": "D",
                    "scenario": null
                }
            ]
        },
        {
            "parameter": "ETP-fw",
            "values": [
                {
                    "value": null,
                    "module": "A1-A3",
                    "scenario": null
                },
                {
                    "value": null,
                    "module": "C2",
                    "scenario": null
                },
                {
                    "value": null,
                    "module": "C3",
                    "scenario": null
                },
                {
                    "value": null,
                    "module": "C4",
                    "scenario": null
                },
                {
                    "value": null,
                    "module": "D",
                    "scenario": null
                }
            ]
        },
        {
            "parameter": "HTP-c",
            "values": [
                {
                    "value": null,
                    "module": "A1-A3",
                    "scenario": null
                },
                {
                    "value": null,
                    "module": "C2",
                    "scenario": null
                },
                {
                    "value": null,
                    "module": "C3",
                    "scenario": null
                },
                {
                    "value": null,
                    "module": "C4",
                    "scenario": null
                },
                {
                    "value": null,
                    "module": "D",
                    "scenario": null
                }
            ]
        },
        {
            "parameter": "HTP-nc",
            "values": [
                {
                    "value": null,
                    "module": "A1-A3",
                    "scenario": null
                },
                {
                    "value": null,
                    "module": "C2",
                    "scenario": null
                },
                {
                    "value": null,
                    "module": "C3",
                    "scenario": null
                },
                {
                    "value": null,
                    "module": "C4",
                    "scenario": null
                },
                {
                    "value": null,
                    "module": "D",
                    "scenario": null
                }
            ]
        },
        {
            "parameter": "SQP",
            "values": [
                {
                    "value": null,
                    "module": "A1-A3",
                    "scenario": null
                },
                {
                    "value": null,
                    "module": "C2",
                    "scenario": null
                },
                {
                    "value": null,
                    "module": "C3",
                    "scenario": null
                },
                {
                    "value": null,
                    "module": "C4",
                    "scenario": null
                },
                {
                    "value": null,
                    "module": "D",
                    "scenario": null
                }
            ]
        },
        {
            "parameter": "IRP",
            "values": [
                {
                    "value": null,
                    "module": "A1-A3",
                    "scenario": null
                },
                {
                    "value": null,
                    "module": "C2",
                    "scenario": null
                },
                {
                    "value": null,
                    "module": "C3",
                    "scenario": null
                },
                {
                    "value": null,
                    "module": "C4",
                    "scenario": null
                },
                {
                    "value": null,
                    "module": "D",
                    "scenario": null
                }
            ]
        }
    ],
    "resource_use": [
        {
            "parameter": "PERE",
            "values": [
                {
                    "value": "1,35E+03",
                    "module": "A1-A3",
                    "scenario": null
                },
                {
                    "value": "8,14E-01",
                    "module": "C2",
                    "scenario": null
                },
                {
                    "value": "1,69E+01",
                    "module": "C3",
                    "scenario": null
                },
                {
                    "value": "0,00E+00",
                    "module": "C4",
                    "scenario": null
                },
                {
                    "value": "-4,47E+02",
                    "module": "D",
                    "scenario": null
                }
            ]
        },
        {
            "parameter": "PERM",
            "values": [
                {
                    "value": "5,39E+01",
                    "module": "A1-A3",
                    "scenario": null
                },
                {
                    "value": "0,00E+00",
                    "module": "C2",
                    "scenario": null
                },
                {
                    "value": "0,00E+00",
                    "module": "C3",
                    "scenario": null
                },
                {
                    "value": "0,00E+00",
                    "module": "C4",
                    "scenario": null
                },
                {
                    "value": "0,00E+00",
                    "module": "D",
                    "scenario": null
                }
            ]
        },
        {
            "parameter": "PERT",
            "values": [
                {
                    "value": "1,40E+03",
                    "module": "A1-A3",
                    "scenario": null
                },
                {
                    "value": "8,14E-01",
                    "module": "C2",
                    "scenario": null
                },
                {
                    "value": "1,69E+01",
                    "module": "C3",
                    "scenario": null
                },
                {
                    "value": "0,00E+00",
                    "module": "C4",
                    "scenario": null
                },
                {
                    "value": "-4,47E+02",
                    "module": "D",
                    "scenario": null
                }
            ]
        },
        {
            "parameter": "PENRE",
            "values": [
                {
                    "value": "1,99E+04",
                    "module": "A1-A3",
                    "scenario": null
                },
                {
                    "value": "3,12E+02",
                    "module": "C2",
                    "scenario": null
                },
                {
                    "value": "1,93E+02",
                    "module": "C3",
                    "scenario": null
                },
                {
                    "value": "0,00E+00",
                    "module": "C4",
                    "scenario": null
                },
                {
                    "value": "-7,51E+03",
                    "module": "D",
                    "scenario": null
                }
            ]
        },
        {
            "parameter": "PENRM",
            "values": [
                {
                    "value": "4,56E+01",
                    "module": "A1-A3",
                    "scenario": null
                },
                {
                    "value": "0,00E+00",
                    "module": "C2",
                    "scenario": null
                },
                {
                    "value": "0,00E+00",
                    "module": "C3",
                    "scenario": null
                },
                {
                    "value": "0,00E+00",
                    "module": "C4",
                    "scenario": null
                },
                {
                    "value": "0,00E+00",
                    "module": "D",
                    "scenario": null
                }
            ]
        },
        {
            "parameter": "PENRT",
            "values": [
                {
                    "value": "2,00E+04",
                    "module": "A1-A3",
                    "scenario": null
                },
                {
                    "value": "3,12E+02",
                    "module": "C2",
                    "scenario": null
                },
                {
                    "value": "1,93E+02",
                    "module": "C3",
                    "scenario": null
                },
                {
                    "value": "0,00E+00",
                    "module": "C4",
                    "scenario": null
                },
                {
                    "value": "-7,51E+03",
                    "module": "D",
                    "scenario": null
                }
            ]
        },
        {
            "parameter": "SM",
            "values": [
                {
                    "value": "4,37E+02",
                    "module": "A1-A3",
                    "scenario": null
                },
                {
                    "value": "0,00E+00",
                    "module": "C2",
                    "scenario": null
                },
                {
                    "value": "0,00E+00",
                    "module": "C3",
                    "scenario": null
                },
                {
                    "value": "0,00E+00",
                    "module": "C4",
                    "scenario": null
                },
                {
                    "value": "6,01E+02",
                    "module": "D",
                    "scenario": null
                }
            ]
        },
        {
            "parameter": "RSF",
            "values": [
                {
                    "value": "0,00E+00",
                    "module": "A1-A3",
                    "scenario": null
                },
                {
                    "value": "0,00E+00",
                    "module": "C2",
                    "scenario": null
                },
                {
                    "value": "0,00E+00",
                    "module": "C3",
                    "scenario": null
                },
                {
                    "value": "0,00E+00",
                    "module": "C4",
                    "scenario": null
                },
                {
                    "value": "0,00E+00",
                    "module": "D",
                    "scenario": null
                }
            ]
        },
        {
            "parameter": "NRSF",
            "values": [
                {
                    "value": "0,00E+00",
                    "module": "A1-A3",
                    "scenario": null
                },
                {
                    "value": "0,00E+00",
                    "module": "C2",
                    "scenario": null
                },
                {
                    "value": "0,00E+00",
                    "module": "C3",
                    "scenario": null
                },
                {
                    "value": "0,00E+00",
                    "module": "C4",
                    "scenario": null
                },
                {
                    "value": "0,00E+00",
                    "module": "D",
                    "scenario": null
                }
            ]
        },
        {
            "parameter": "FW",
            "values": [
                {
                    "value": "7,17E+00",
                    "module": "A1-A3",
                    "scenario": null
                },
                {
                    "value": "1,31E-02",
                    "module": "C2",
                    "scenario": null
                },
                {
                    "value": "3,52E-02",
                    "module": "C3",
                    "scenario": null
                },
                {
                    "value": "0,00E+00",
                    "module": "C4",
                    "scenario": null
                },
                {
                    "value": "-2,50E+00",
                    "module": "D",
                    "scenario": null
                }
            ]
        }
    ],
    "end_of_life_waste": [
        {
            "parameter": "HWD",
            "values": [
                {
                    "value": "6,97E-01",
                    "module": "A1-A3",
                    "scenario": null
                },
                {
                    "value": null,
                    "module": "C2",
                    "scenario": null
                },
                {
                    "value": null,
                    "module": "C3",
                    "scenario": null
                },
                {
                    "value": "0,00E+00",
                    "module": "C4",
                    "scenario": null
                },
                {
                    "value": null,
                    "module": "D",
                    "scenario": null
                }
            ]
        },
        {
            "parameter": "NHWD",
            "values": [
                {
                    "value": "0,00E+00",
                    "module": "A1-A3",
                    "scenario": null
                },
                {
                    "value": null,
                    "module": "C2",
                    "scenario": null
                },
                {
                    "value": null,
                    "module": "C3",
                    "scenario": null
                },
                {
                    "value": "0,00E+00",
                    "module": "C4",
                    "scenario": null
                },
                {
                    "value": null,
                    "module": "D",
                    "scenario": null
                }
            ]
        },
        {
            "parameter": "RWD",
            "values": [
                {
                    "value": "0,00E+00",
                    "module": "A1-A3",
                    "scenario": null
                },
                {
                    "value": null,
                    "module": "C2",
                    "scenario": null
                },
                {
                    "value": null,
                    "module": "C3",
                    "scenario": null
                },
                {
                    "value": "0,00E+00",
                    "module": "C4",
                    "scenario": null
                },
                {
                    "value": null,
                    "module": "D",
                    "scenario": null
                }
            ]
        }
    ],
    "end_of_life_flow": [
        {
            "parameter": "CRU",
            "values": [
                {
                    "value": "0,00E+00",
                    "module": "A1-A3",
                    "scenario": null
                },
                {
                    "value": null,
                    "module": "C2",
                    "scenario": null
                },
                {
                    "value": "0,00E+00",
                    "module": "C3",
                    "scenario": null
                },
                {
                    "value": "0,00E+00",
                    "module": "C4",
                    "scenario": null
                },
                {
                    "value": null,
                    "module": "D",
                    "scenario": null
                }
            ]
        },
        {
            "parameter": "MFR",
            "values": [
                {
                    "value": "3,82E+01",
                    "module": "A1-A3",
                    "scenario": null
                },
                {
                    "value": null,
                    "module": "C2",
                    "scenario": null
                },
                {
                    "value": "1,00E+03",
                    "module": "C3",
                    "scenario": null
                },
                {
                    "value": "0,00E+00",
                    "module": "C4",
                    "scenario": null
                },
                {
                    "value": null,
                    "module": "D",
                    "scenario": null
                }
            ]
        },
        {
            "parameter": "MER",
            "values": [
                {
                    "value": "0,00E+00",
                    "module": "A1-A3",
                    "scenario": null
                },
                {
                    "value": null,
                    "module": "C2",
                    "scenario": null
                },
                {
                    "value": "0,00E+00",
                    "module": "C3",
                    "scenario": null
                },
                {
                    "value": "0,00E+00",
                    "module": "C4",
                    "scenario": null
                },
                {
                    "value": null,
                    "module": "D",
                    "scenario": null
                }
            ]
        },
        {
            "parameter": "EEE",
            "values": [
                {
                    "value": "0,00E+00",
                    "module": "A1-A3",
                    "scenario": null
                },
                {
                    "value": null,
                    "module": "C2",
                    "scenario": null
                },
                {
                    "value": "0,00E+00",
                    "module": "C3",
                    "scenario": null
                },
                {
                    "value": "0,00E+00",
                    "module": "C4",
                    "scenario": null
                },
                {
                    "value": null,
                    "module": "D",
                    "scenario": null
                }
            ]
        },
        {
            "parameter": "EET",
            "values": [
                {
                    "value": "0,00E+00",
                    "module": "A1-A3",
                    "scenario": null
                },
                {
                    "value": null,
                    "module": "C2",
                    "scenario": null
                },
                {
                    "value": "0,00E+00",
                    "module": "C3",
                    "scenario": null
                },
                {
                    "value": "0,00E+00",
                    "module": "C4",
                    "scenario": null
                },
                {
                    "value": null,
                    "module": "D",
                    "scenario": null
                }
            ]
        }
    ]
}