{
    "product_name": "Tufted modular carpet tiles with CQuest Bio backing, aqueous dyed surface and a max. total pile material of 1500 g/m\u00b2 PA 6 with 100% recycled content",
    "epd_id": "EPD-INT-20210152-CBB2-EN",
    "declared_unit": {
        "unit": "m2",
        "amount": 1.0
    },
    "compliance": [
        "DIN EN 15804",
        "ISO 14025"
    ],
    "producer_name": "Interface Europe Manufacturing BV",
    "environmental_impact": [
        {
            "parameter": "GWP-total",
            "values": [
                {
                    "value": "5,26E+00",
                    "module": "A1-A3",
                    "scenario": null
                },
                {
                    "value": "3,19E-01",
                    "module": "A4",
                    "scenario": null
                },
                {
                    "value": "5,93E-01",
                    "module": "A5",
                    "scenario": null
                },
                {
                    "value": "0,00E+00",
                    "module": "B1",
                    "scenario": null
                },
                {
                    "value": "2,91E-01",
                    "module": "B2",
                    "scenario": null
                },
                {
                    "value": "4,45E-02",
                    "module": "C2",
                    "scenario": null
                },
                {
                    "value": "7,03E+00",
                    "module": "C3",
                    "scenario": "S2"
                },
                {
                    "value": "7,11E+00",
                    "module": "C3",
                    "scenario": "S3"
                },
                {
                    "value": "1,26E+00",
                    "module": "C4",
                    "scenario": null
                },
                {
                    "value": "-1,95E-02",
                    "module": "D",
                    "scenario": "S0"
                },
                {
                    "value": "0,00E+00",
                    "module": "D",
                    "scenario": "S1"
                },
                {
                    "value": "-3,27E-01",
                    "module": "D",
                    "scenario": "S2"
                },
                {
                    "value": "-2,41E-01",
                    "module": "D",
                    "scenario": "S3"
                }
            ]
        },
        {
            "parameter": "ODP",
            "values": [
                {
                    "value": "2,74E-08",
                    "module": "A1-A3",
                    "scenario": null
                },
                {
                    "value": "5,56E-17",
                    "module": "A4",
                    "scenario": null
                },
                {
                    "value": "8,22E-10",
                    "module": "A5",
                    "scenario": null
                },
                {
                    "value": "0,00E+00",
                    "module": "B1",
                    "scenario": null
                },
                {
                    "value": "1,21E-08",
                    "module": "B2",
                    "scenario": null
                },
                {
                    "value": "7,76E-18",
                    "module": "C2",
                    "scenario": null
                },
                {
                    "value": "2,55E-15",
                    "module": "C3",
                    "scenario": "S2"
                },
                {
                    "value": "3,50E-15",
                    "module": "C3",
                    "scenario": "S3"
                },
                {
                    "value": "1,23E-15",
                    "module": "C4",
                    "scenario": null
                },
                {
                    "value": "-2,99E-16",
                    "module": "D",
                    "scenario": "S0"
                },
                {
                    "value": "0,00E+00",
                    "module": "D",
                    "scenario": "S1"
                },
                {
                    "value": "-4,93E-15",
                    "module": "D",
                    "scenario": "S2"
                },
                {
                    "value": "-1,46E-15",
                    "module": "D",
                    "scenario": "S3"
                }
            ]
        },
        {
            "parameter": "AP",
            "values": [
                {
                    "value": "2,33E-02",
                    "module": "A1-A3",
                    "scenario": null
                },
                {
                    "value": "1,32E-03",
                    "module": "A4",
                    "scenario": null
                },
                {
                    "value": "8,93E-04",
                    "module": "A5",
                    "scenario": null
                },
                {
                    "value": "0,00E+00",
                    "module": "B1",
                    "scenario": null
                },
                {
                    "value": "1,14E-03",
                    "module": "B2",
                    "scenario": null
                },
                {
                    "value": "1,84E-04",
                    "module": "C2",
                    "scenario": null
                },
                {
                    "value": "4,99E-03",
                    "module": "C3",
                    "scenario": "S2"
                },
                {
                    "value": "5,24E-03",
                    "module": "C3",
                    "scenario": "S3"
                },
                {
                    "value": "9,44E-04",
                    "module": "C4",
                    "scenario": null
                },
                {
                    "value": "-2,27E-05",
                    "module": "D",
                    "scenario": "S0"
                },
                {
                    "value": "0,00E+00",
                    "module": "D",
                    "scenario": "S1"
                },
                {
                    "value": "-3,75E-04",
                    "module": "D",
                    "scenario": "S2"
                },
                {
                    "value": "-8,63E-04",
                    "module": "D",
                    "scenario": "S3"
                }
            ]
        },
        {
            "parameter": "EP",
            "values": [
                {
                    "value": "5,95E-03",
                    "module": "A1-A3",
                    "scenario": null
                },
                {
                    "value": "3,36E-04",
                    "module": "A4",
                    "scenario": null
                },
                {
                    "value": "2,27E-04",
                    "module": "A5",
                    "scenario": null
                },
                {
                    "value": "0,00E+00",
                    "module": "B1",
                    "scenario": null
                },
                {
                    "value": "3,16E-04",
                    "module": "B2",
                    "scenario": null
                },
                {
                    "value": "4,68E-05",
                    "module": "C2",
                    "scenario": null
                },
                {
                    "value": "1,26E-03",
                    "module": "C3",
                    "scenario": "S2"
                },
                {
                    "value": "1,31E-03",
                    "module": "C3",
                    "scenario": "S3"
                },
                {
                    "value": "1,03E-03",
                    "module": "C4",
                    "scenario": null
                },
                {
                    "value": "-3,11E-06",
                    "module": "D",
                    "scenario": "S0"
                },
                {
                    "value": "0,00E+00",
                    "module": "D",
                    "scenario": "S1"
                },
                {
                    "value": "-5,17E-05",
                    "module": "D",
                    "scenario": "S2"
                },
                {
                    "value": "-1,13E-04",
                    "module": "D",
                    "scenario": "S3"
                }
            ]
        },
        {
            "parameter": "POCP",
            "values": [
                {
                    "value": "1,42E-03",
                    "module": "A1-A3",
                    "scenario": null
                },
                {
                    "value": "-5,64E-04",
                    "module": "A4",
                    "scenario": null
                },
                {
                    "value": "3,37E-05",
                    "module": "A5",
                    "scenario": null
                },
                {
                    "value": "6,29E-05",
                    "module": "B1",
                    "scenario": null
                },
                {
                    "value": "1,47E-04",
                    "module": "B2",
                    "scenario": null
                },
                {
                    "value": "-7,88E-05",
                    "module": "C2",
                    "scenario": null
                },
                {
                    "value": "3,03E-04",
                    "module": "C3",
                    "scenario": "S2"
                },
                {
                    "value": "2,28E-04",
                    "module": "C3",
                    "scenario": "S3"
                },
                {
                    "value": "8,50E-05",
                    "module": "C4",
                    "scenario": null
                },
                {
                    "value": "-2,08E-06",
                    "module": "D",
                    "scenario": "S0"
                },
                {
                    "value": "0,00E+00",
                    "module": "D",
                    "scenario": "S1"
                },
                {
                    "value": "-3,46E-05",
                    "module": "D",
                    "scenario": "S2"
                },
                {
                    "value": "-8,03E-05",
                    "module": "D",
                    "scenario": "S3"
                }
            ]
        },
        {
            "parameter": "ADPE",
            "values": [
                {
                    "value": "9,95E-06",
                    "module": "A1-A3",
                    "scenario": null
                },
                {
                    "value": "2,83E-08",
                    "module": "A4",
                    "scenario": null
                },
                {
                    "value": "3,06E-07",
                    "module": "A5",
                    "scenario": null
                },
                {
                    "value": "0,00E+00",
                    "module": "B1",
                    "scenario": null
                },
                {
                    "value": "4,43E-06",
                    "module": "B2",
                    "scenario": null
                },
                {
                    "value": "3,94E-09",
                    "module": "C2",
                    "scenario": null
                },
                {
                    "value": "2,31E-07",
                    "module": "C3",
                    "scenario": "S2"
                },
                {
                    "value": "2,45E-07",
                    "module": "C3",
                    "scenario": "S3"
                },
                {
                    "value": "6,98E-08",
                    "module": "C4",
                    "scenario": null
                },
                {
                    "value": "-3,67E-09",
                    "module": "D",
                    "scenario": "S0"
                },
                {
                    "value": "0,00E+00",
                    "module": "D",
                    "scenario": "S1"
                },
                {
                    "value": "-6,07E-08",
                    "module": "D",
                    "scenario": "S2"
                },
                {
                    "value": "-1,90E-07",
                    "module": "D",
                    "scenario": "S3"
                }
            ]
        },
        {
            "parameter": "ADPF",
            "values": [
                {
                    "value": "1,07E+02",
                    "module": "A1-A3",
                    "scenario": null
                },
                {
                    "value": "4,34E+00",
                    "module": "A4",
                    "scenario": null
                },
                {
                    "value": "3,48E+00",
                    "module": "A5",
                    "scenario": null
                },
                {
                    "value": "0,00E+00",
                    "module": "B1",
                    "scenario": null
                },
                {
                    "value": "6,77E+00",
                    "module": "B2",
                    "scenario": null
                },
                {
                    "value": "6,06E-01",
                    "module": "C2",
                    "scenario": null
                },
                {
                    "value": "3,85E+00",
                    "module": "C3",
                    "scenario": "S2"
                },
                {
                    "value": "4,79E+00",
                    "module": "C3",
                    "scenario": "S3"
                },
                {
                    "value": "5,44E+00",
                    "module": "C4",
                    "scenario": null
                },
                {
                    "value": "-2,81E-01",
                    "module": "D",
                    "scenario": "S0"
                },
                {
                    "value": "0,00E+00",
                    "module": "D",
                    "scenario": "S1"
                },
                {
                    "value": "-4,71E+00",
                    "module": "D",
                    "scenario": "S2"
                },
                {
                    "value": "-2,16E+01",
                    "module": "D",
                    "scenario": "S3"
                }
            ]
        }
    ],
    "additional_environmental_impact": [],
    "resource_use": [
        {
            "parameter": "PERE",
            "values": [
                {
                    "value": "8,49E+01",
                    "module": "A1-A3",
                    "scenario": null
                },
                {
                    "value": "2,43E-01",
                    "module": "A4",
                    "scenario": null
                },
                {
                    "value": "3,37E+00",
                    "module": "A5",
                    "scenario": null
                },
                {
                    "value": "0,00E+00",
                    "module": "B1",
                    "scenario": null
                },
                {
                    "value": "1,24E+00",
                    "module": "B2",
                    "scenario": null
                },
                {
                    "value": "3,38E-02",
                    "module": "C2",
                    "scenario": null
                },
                {
                    "value": "1,47E+01",
                    "module": "C3",
                    "scenario": "S2"
                },
                {
                    "value": "1,49E+01",
                    "module": "C3",
                    "scenario": "S3"
                },
                {
                    "value": "4,06E-01",
                    "module": "C4",
                    "scenario": null
                },
                {
                    "value": "-7,71E-02",
                    "module": "D",
                    "scenario": "S0"
                },
                {
                    "value": "0,00E+00",
                    "module": "D",
                    "scenario": "S1"
                },
                {
                    "value": "-1,27E+00",
                    "module": "D",
                    "scenario": "S2"
                },
                {
                    "value": "-3,42E-01",
                    "module": "D",
                    "scenario": "S3"
                }
            ]
        },
        {
            "parameter": "PERM",
            "values": [
                {
                    "value": "1,44E+01",
                    "module": "A1-A3",
                    "scenario": null
                },
                {
                    "value": "0,00E+00",
                    "module": "A4",
                    "scenario": null
                },
                {
                    "value": "-3,63E-01",
                    "module": "A5",
                    "scenario": null
                },
                {
                    "value": "0,00E+00",
                    "module": "B1",
                    "scenario": null
                },
                {
                    "value": "0,00E+00",
                    "module": "B2",
                    "scenario": null
                },
                {
                    "value": "0,00E+00",
                    "module": "C2",
                    "scenario": null
                },
                {
                    "value": "-1,41E+01",
                    "module": "C3",
                    "scenario": "S2"
                },
                {
                    "value": "-1,41E+01",
                    "module": "C3",
                    "scenario": "S3"
                },
                {
                    "value": "0,00E+00",
                    "module": "C4",
                    "scenario": null
                },
                {
                    "value": "0,00E+00",
                    "module": "D",
                    "scenario": "S0"
                },
                {
                    "value": "0,00E+00",
                    "module": "D",
                    "scenario": "S1"
                },
                {
                    "value": "0,00E+00",
                    "module": "D",
                    "scenario": "S2"
                },
                {
                    "value": "0,00E+00",
                    "module": "D",
                    "scenario": "S3"
                }
            ]
        },
        {
            "parameter": "PERT",
            "values": [
                {
                    "value": "9,94E+01",
                    "module": "A1-A3",
                    "scenario": null
                },
                {
                    "value": "2,43E-01",
                    "module": "A4",
                    "scenario": null
                },
                {
                    "value": "3,01E+00",
                    "module": "A5",
                    "scenario": null
                },
                {
                    "value": "0,00E+00",
                    "module": "B1",
                    "scenario": null
                },
                {
                    "value": "1,24E+00",
                    "module": "B2",
                    "scenario": null
                },
                {
                    "value": "3,38E-02",
                    "module": "C2",
                    "scenario": null
                },
                {
                    "value": "5,99E-01",
                    "module": "C3",
                    "scenario": "S2"
                },
                {
                    "value": "8,75E-01",
                    "module": "C3",
                    "scenario": "S3"
                },
                {
                    "value": "4,06E-01",
                    "module": "C4",
                    "scenario": null
                },
                {
                    "value": "-7,71E-02",
                    "module": "D",
                    "scenario": "S0"
                },
                {
                    "value": "0,00E+00",
                    "module": "D",
                    "scenario": "S1"
                },
                {
                    "value": "-1,27E+00",
                    "module": "D",
                    "scenario": "S2"
                },
                {
                    "value": "-3,42E-01",
                    "module": "D",
                    "scenario": "S3"
                }
            ]
        },
        {
            "parameter": "PENRE",
            "values": [
                {
                    "value": "1,05E+02",
                    "module": "A1-A3",
                    "scenario": null
                },
                {
                    "value": "4,35E+00",
                    "module": "A4",
                    "scenario": null
                },
                {
                    "value": "3,95E+00",
                    "module": "A5",
                    "scenario": null
                },
                {
                    "value": "0,00E+00",
                    "module": "B1",
                    "scenario": null
                },
                {
                    "value": "7,86E+00",
                    "module": "B2",
                    "scenario": null
                },
                {
                    "value": "6,07E-01",
                    "module": "C2",
                    "scenario": null
                },
                {
                    "value": "1,29E+01",
                    "module": "C3",
                    "scenario": "S2"
                },
                {
                    "value": "1,40E+01",
                    "module": "C3",
                    "scenario": "S3"
                },
                {
                    "value": "5,60E+00",
                    "module": "C4",
                    "scenario": null
                },
                {
                    "value": "-3,43E-01",
                    "module": "D",
                    "scenario": "S0"
                },
                {
                    "value": "0,00E+00",
                    "module": "D",
                    "scenario": "S1"
                },
                {
                    "value": "-5,74E+00",
                    "module": "D",
                    "scenario": "S2"
                },
                {
                    "value": "-2,18E+01",
                    "module": "D",
                    "scenario": "S3"
                }
            ]
        },
        {
            "parameter": "PENRM",
            "values": [
                {
                    "value": "8,95E+00",
                    "module": "A1-A3",
                    "scenario": null
                },
                {
                    "value": "0,00E+00",
                    "module": "A4",
                    "scenario": null
                },
                {
                    "value": "-2,75E-01",
                    "module": "A5",
                    "scenario": null
                },
                {
                    "value": "0,00E+00",
                    "module": "B1",
                    "scenario": null
                },
                {
                    "value": "0,00E+00",
                    "module": "B2",
                    "scenario": null
                },
                {
                    "value": "0,00E+00",
                    "module": "C2",
                    "scenario": null
                },
                {
                    "value": "-8,68E+00",
                    "module": "C3",
                    "scenario": "S2"
                },
                {
                    "value": "-8,68E+00",
                    "module": "C3",
                    "scenario": "S3"
                },
                {
                    "value": "0,00E+00",
                    "module": "C4",
                    "scenario": null
                },
                {
                    "value": "0,00E+00",
                    "module": "D",
                    "scenario": "S0"
                },
                {
                    "value": "0,00E+00",
                    "module": "D",
                    "scenario": "S1"
                },
                {
                    "value": "0,00E+00",
                    "module": "D",
                    "scenario": "S2"
                },
                {
                    "value": "0,00E+00",
                    "module": "D",
                    "scenario": "S3"
                }
            ]
        },
        {
            "parameter": "PENRT",
            "values": [
                {
                    "value": "1,14E+02",
                    "module": "A1-A3",
                    "scenario": null
                },
                {
                    "value": "4,35E+00",
                    "module": "A4",
                    "scenario": null
                },
                {
                    "value": "3,67E+00",
                    "module": "A5",
                    "scenario": null
                },
                {
                    "value": "0,00E+00",
                    "module": "B1",
                    "scenario": null
                },
                {
                    "value": "7,86E+00",
                    "module": "B2",
                    "scenario": null
                },
                {
                    "value": "6,07E-01",
                    "module": "C2",
                    "scenario": null
                },
                {
                    "value": "4,21E+00",
                    "module": "C3",
                    "scenario": "S2"
                },
                {
                    "value": "5,34E+00",
                    "module": "C3",
                    "scenario": "S3"
                },
                {
                    "value": "5,60E+00",
                    "module": "C4",
                    "scenario": null
                },
                {
                    "value": "-3,43E-01",
                    "module": "D",
                    "scenario": "S0"
                },
                {
                    "value": "0,00E+00",
                    "module": "D",
                    "scenario": "S1"
                },
                {
                    "value": "-5,74E+00",
                    "module": "D",
                    "scenario": "S2"
                },
                {
                    "value": "-2,18E+01",
                    "module": "D",
                    "scenario": "S3"
                }
            ]
        },
        {
            "parameter": "SM",
            "values": [
                {
                    "value": "4,28E+00",
                    "module": "A1-A3",
                    "scenario": null
                },
                {
                    "value": "0,00E+00",
                    "module": "A4",
                    "scenario": null
                },
                {
                    "value": "1,28E-01",
                    "module": "A5",
                    "scenario": null
                },
                {
                    "value": "0,00E+00",
                    "module": "B1",
                    "scenario": null
                },
                {
                    "value": "0,00E+00",
                    "module": "B2",
                    "scenario": null
                },
                {
                    "value": "0,00E+00",
                    "module": "C2",
                    "scenario": null
                },
                {
                    "value": "0,00E+00",
                    "module": "C3",
                    "scenario": "S2"
                },
                {
                    "value": "0,00E+00",
                    "module": "C3",
                    "scenario": "S3"
                },
                {
                    "value": "0,00E+00",
                    "module": "C4",
                    "scenario": null
                },
                {
                    "value": "0,00E+00",
                    "module": "D",
                    "scenario": "S0"
                },
                {
                    "value": "0,00E+00",
                    "module": "D",
                    "scenario": "S1"
                },
                {
                    "value": "0,00E+00",
                    "module": "D",
                    "scenario": "S2"
                },
                {
                    "value": "2,60E-01",
                    "module": "D",
                    "scenario": "S3"
                }
            ]
        },
        {
            "parameter": "RSF",
            "values": [
                {
                    "value": "0,00E+00",
                    "module": "A1-A3",
                    "scenario": null
                },
                {
                    "value": "0,00E+00",
                    "module": "A4",
                    "scenario": null
                },
                {
                    "value": "0,00E+00",
                    "module": "A5",
                    "scenario": null
                },
                {
                    "value": "0,00E+00",
                    "module": "B1",
                    "scenario": null
                },
                {
                    "value": "0,00E+00",
                    "module": "B2",
                    "scenario": null
                },
                {
                    "value": "0,00E+00",
                    "module": "C2",
                    "scenario": null
                },
                {
                    "value": "0,00E+00",
                    "module": "C3",
                    "scenario": "S2"
                },
                {
                    "value": "0,00E+00",
                    "module": "C3",
                    "scenario": "S3"
                },
                {
                    "value": "0,00E+00",
                    "module": "C4",
                    "scenario": null
                },
                {
                    "value": "0,00E+00",
                    "module": "D",
                    "scenario": "S0"
                },
                {
                    "value": "0,00E+00",
                    "module": "D",
                    "scenario": "S1"
                },
                {
                    "value": "0,00E+00",
                    "module": "D",
                    "scenario": "S2"
                },
                {
                    "value": "0,00E+00",
                    "module": "D",
                    "scenario": "S3"
                }
            ]
        },
        {
            "parameter": "NRSF",
            "values": [
                {
                    "value": "0,00E+00",
                    "module": "A1-A3",
                    "scenario": null
                },
                {
                    "value": "0,00E+00",
                    "module": "A4",
                    "scenario": null
                },
                {
                    "value": "0,00E+00",
                    "module": "A5",
                    "scenario": null
                },
                {
                    "value": "0,00E+00",
                    "module": "B1",
                    "scenario": null
                },
                {
                    "value": "0,00E+00",
                    "module": "B2",
                    "scenario": null
                },
                {
                    "value": "0,00E+00",
                    "module": "C2",
                    "scenario": null
                },
                {
                    "value": "0,00E+00",
                    "module": "C3",
                    "scenario": "S2"
                },
                {
                    "value": "0,00E+00",
                    "module": "C3",
                    "scenario": "S3"
                },
                {
                    "value": "0,00E+00",
                    "module": "C4",
                    "scenario": null
                },
                {
                    "value": "0,00E+00",
                    "module": "D",
                    "scenario": "S0"
                },
                {
                    "value": "0,00E+00",
                    "module": "D",
                    "scenario": "S1"
                },
                {
                    "value": "0,00E+00",
                    "module": "D",
                    "scenario": "S2"
                },
                {
                    "value": "0,00E+00",
                    "module": "D",
                    "scenario": "S3"
                }
            ]
        },
        {
            "parameter": "FW",
            "values": [
                {
                    "value": "4,93E-01",
                    "module": "A1-A3",
                    "scenario": null
                },
                {
                    "value": "2,78E-04",
                    "module": "A4",
                    "scenario": null
                },
                {
                    "value": "1,55E-02",
                    "module": "A5",
                    "scenario": null
                },
                {
                    "value": "0,00E+00",
                    "module": "B1",
                    "scenario": null
                },
                {
                    "value": "4,13E-03",
                    "module": "B2",
                    "scenario": null
                },
                {
                    "value": "3,87E-05",
                    "module": "C2",
                    "scenario": null
                },
                {
                    "value": "2,03E-02",
                    "module": "C3",
                    "scenario": "S2"
                },
                {
                    "value": "2,06E-02",
                    "module": "C3",
                    "scenario": "S3"
                },
                {
                    "value": "5,16E-05",
                    "module": "C4",
                    "scenario": null
                },
                {
                    "value": "-7,53E-05",
                    "module": "D",
                    "scenario": "S0"
                },
                {
                    "value": "0,00E+00",
                    "module": "D",
                    "scenario": "S1"
                },
                {
                    "value": "-1,24E-03",
                    "module": "D",
                    "scenario": "S2"
                },
                {
                    "value": "-2,06E-03",
                    "module": "D",
                    "scenario": "S3"
                }
            ]
        }
    ],
    "end_of_life_waste": [
        {
            "parameter": "HWD",
            "values": [
                {
                    "value": "4,23E-03",
                    "module": "A1-A3",
                    "scenario": null
                },
                {
                    "value": "2,19E-10",
                    "module": "A4",
                    "scenario": null
                },
                {
                    "value": "1,27E-04",
                    "module": "A5",
                    "scenario": null
                },
                {
                    "value": "0,00E+00",
                    "module": "B1",
                    "scenario": null
                },
                {
                    "value": "5,90E-10",
                    "module": "B2",
                    "scenario": null
                },
                {
                    "value": "3,06E-11",
                    "module": "C2",
                    "scenario": null
                },
                {
                    "value": "1,69E-08",
                    "module": "C3",
                    "scenario": "S2"
                },
                {
                    "value": "1,71E-08",
                    "module": "C3",
                    "scenario": "S3"
                },
                {
                    "value": "1,01E-09",
                    "module": "C4",
                    "scenario": null
                },
                {
                    "value": "-7,70E-11",
                    "module": "D",
                    "scenario": "S0"
                },
                {
                    "value": "0,00E+00",
                    "module": "D",
                    "scenario": "S1"
                },
                {
                    "value": "-1,29E-09",
                    "module": "D",
                    "scenario": "S2"
                },
                {
                    "value": "-1,67E-09",
                    "module": "D",
                    "scenario": "S3"
                }
            ]
        },
        {
            "parameter": "NHWD",
            "values": [
                {
                    "value": "8,09E-01",
                    "module": "A1-A3",
                    "scenario": null
                },
                {
                    "value": "6,47E-04",
                    "module": "A4",
                    "scenario": null
                },
                {
                    "value": "6,87E-02",
                    "module": "A5",
                    "scenario": null
                },
                {
                    "value": "0,00E+00",
                    "module": "B1",
                    "scenario": null
                },
                {
                    "value": "5,62E-03",
                    "module": "B2",
                    "scenario": null
                },
                {
                    "value": "9,02E-05",
                    "module": "C2",
                    "scenario": null
                },
                {
                    "value": "1,48E+00",
                    "module": "C3",
                    "scenario": "S2"
                },
                {
                    "value": "1,48E+00",
                    "module": "C3",
                    "scenario": "S3"
                },
                {
                    "value": "5,34E+00",
                    "module": "C4",
                    "scenario": null
                },
                {
                    "value": "-1,60E-04",
                    "module": "D",
                    "scenario": "S0"
                },
                {
                    "value": "0,00E+00",
                    "module": "D",
                    "scenario": "S1"
                },
                {
                    "value": "-2,67E-03",
                    "module": "D",
                    "scenario": "S2"
                },
                {
                    "value": "-1,62E-01",
                    "module": "D",
                    "scenario": "S3"
                }
            ]
        },
        {
            "parameter": "RWD",
            "values": [
                {
                    "value": "2,19E-03",
                    "module": "A1-A3",
                    "scenario": null
                },
                {
                    "value": "5,27E-06",
                    "module": "A4",
                    "scenario": null
                },
                {
                    "value": "7,03E-05",
                    "module": "A5",
                    "scenario": null
                },
                {
                    "value": "0,00E+00",
                    "module": "B1",
                    "scenario": null
                },
                {
                    "value": "3,31E-04",
                    "module": "B2",
                    "scenario": null
                },
                {
                    "value": "7,35E-07",
                    "module": "C2",
                    "scenario": null
                },
                {
                    "value": "1,42E-04",
                    "module": "C3",
                    "scenario": "S2"
                },
                {
                    "value": "2,21E-04",
                    "module": "C3",
                    "scenario": "S3"
                },
                {
                    "value": "6,50E-05",
                    "module": "C4",
                    "scenario": null
                },
                {
                    "value": "-2,48E-05",
                    "module": "D",
                    "scenario": "S0"
                },
                {
                    "value": "0,00E+00",
                    "module": "D",
                    "scenario": "S1"
                },
                {
                    "value": "-4,09E-04",
                    "module": "D",
                    "scenario": "S2"
                },
                {
                    "value": "-8,83E-05",
                    "module": "D",
                    "scenario": "S3"
                }
            ]
        }
    ],
    "end_of_life_flow": [
        {
            "parameter": "CRU",
            "values": [
                {
                    "value": "0,00E+00",
                    "module": "A1-A3",
                    "scenario": null
                },
                {
                    "value": "0,00E+00",
                    "module": "A4",
                    "scenario": null
                },
                {
                    "value": "0,00E+00",
                    "module": "A5",
                    "scenario": null
                },
                {
                    "value": "0,00E+00",
                    "module": "B1",
                    "scenario": null
                },
                {
                    "value": "0,00E+00",
                    "module": "B2",
                    "scenario": null
                },
                {
                    "value": "0,00E+00",
                    "module": "C2",
                    "scenario": null
                },
                {
                    "value": "0,00E+00",
                    "module": "C3",
                    "scenario": "S2"
                },
                {
                    "value": "0,00E+00",
                    "module": "C3",
                    "scenario": "S3"
                },
                {
                    "value": "0,00E+00",
                    "module": "C4",
                    "scenario": null
                },
                {
                    "value": "0,00E+00",
                    "module": "D",
                    "scenario": "S0"
                },
                {
                    "value": "0,00E+00",
                    "module": "D",
                    "scenario": "S1"
                },
                {
                    "value": "0,00E+00",
                    "module": "D",
                    "scenario": "S2"
                },
                {
                    "value": "0,00E+00",
                    "module": "D",
                    "scenario": "S3"
                }
            ]
        },
        {
            "parameter": "MFR",
            "values": [
                {
                    "value": "0,00E+00",
                    "module": "A1-A3",
                    "scenario": null
                },
                {
                    "value": "0,00E+00",
                    "module": "A4",
                    "scenario": null
                },
                {
                    "value": "1,21E-01",
                    "module": "A5",
                    "scenario": null
                },
                {
                    "value": "0,00E+00",
                    "module": "B1",
                    "scenario": null
                },
                {
                    "value": "0,00E+00",
                    "module": "B2",
                    "scenario": null
                },
                {
                    "value": "0,00E+00",
                    "module": "C2",
                    "scenario": null
                },
                {
                    "value": "0,00E+00",
                    "module": "C3",
                    "scenario": "S2"
                },
                {
                    "value": "1,70E+00",
                    "module": "C3",
                    "scenario": "S3"
                },
                {
                    "value": "0,00E+00",
                    "module": "C4",
                    "scenario": null
                },
                {
                    "value": "0,00E+00",
                    "module": "D",
                    "scenario": "S0"
                },
                {
                    "value": "0,00E+00",
                    "module": "D",
                    "scenario": "S1"
                },
                {
                    "value": "0,00E+00",
                    "module": "D",
                    "scenario": "S2"
                },
                {
                    "value": "0,00E+00",
                    "module": "D",
                    "scenario": "S3"
                }
            ]
        },
        {
            "parameter": "MER",
            "values": [
                {
                    "value": "0,00E+00",
                    "module": "A1-A3",
                    "scenario": null
                },
                {
                    "value": "0,00E+00",
                    "module": "A4",
                    "scenario": null
                },
                {
                    "value": "0,00E+00",
                    "module": "A5",
                    "scenario": null
                },
                {
                    "value": "0,00E+00",
                    "module": "B1",
                    "scenario": null
                },
                {
                    "value": "0,00E+00",
                    "module": "B2",
                    "scenario": null
                },
                {
                    "value": "0,00E+00",
                    "module": "C2",
                    "scenario": null
                },
                {
                    "value": "0,00E+00",
                    "module": "C3",
                    "scenario": "S2"
                },
                {
                    "value": "0,00E+00",
                    "module": "C3",
                    "scenario": "S3"
                },
                {
                    "value": "0,00E+00",
                    "module": "C4",
                    "scenario": null
                },
                {
                    "value": "0,00E+00",
                    "module": "D",
                    "scenario": "S0"
                },
                {
                    "value": "0,00E+00",
                    "module": "D",
                    "scenario": "S1"
                },
                {
                    "value": "0,00E+00",
                    "module": "D",
                    "scenario": "S2"
                },
                {
                    "value": "0,00E+00",
                    "module": "D",
                    "scenario": "S3"
                }
            ]
        },
        {
            "parameter": "EEE",
            "values": [
                {
                    "value": "0,00E+00",
                    "module": "A1-A3",
                    "scenario": null
                },
                {
                    "value": "0,00E+00",
                    "module": "A4",
                    "scenario": null
                },
                {
                    "value": "2,78E-01",
                    "module": "A5",
                    "scenario": null
                },
                {
                    "value": "0,00E+00",
                    "module": "B1",
                    "scenario": null
                },
                {
                    "value": "0,00E+00",
                    "module": "B2",
                    "scenario": null
                },
                {
                    "value": "0,00E+00",
                    "module": "C2",
                    "scenario": null
                },
                {
                    "value": "7,85E+00",
                    "module": "C3",
                    "scenario": "S2"
                },
                {
                    "value": "0,00E+00",
                    "module": "C3",
                    "scenario": "S3"
                },
                {
                    "value": "0,00E+00",
                    "module": "C4",
                    "scenario": null
                },
                {
                    "value": "0,00E+00",
                    "module": "D",
                    "scenario": "S0"
                },
                {
                    "value": "0,00E+00",
                    "module": "D",
                    "scenario": "S1"
                },
                {
                    "value": "0,00E+00",
                    "module": "D",
                    "scenario": "S2"
                },
                {
                    "value": "0,00E+00",
                    "module": "D",
                    "scenario": "S3"
                }
            ]
        },
        {
            "parameter": "EET",
            "values": [
                {
                    "value": "0,00E+00",
                    "module": "A1-A3",
                    "scenario": null
                },
                {
                    "value": "0,00E+00",
                    "module": "A4",
                    "scenario": null
                },
                {
                    "value": "5,17E-01",
                    "module": "A5",
                    "scenario": null
                },
                {
                    "value": "0,00E+00",
                    "module": "B1",
                    "scenario": null
                },
                {
                    "value": "0,00E+00",
                    "module": "B2",
                    "scenario": null
                },
                {
                    "value": "0,00E+00",
                    "module": "C2",
                    "scenario": null
                },
                {
                    "value": "1,47E+01",
                    "module": "C3",
                    "scenario": "S2"
                },
                {
                    "value": "7,45E+01",
                    "module": "C3",
                    "scenario": "S3"
                },
                {
                    "value": "0,00E+00",
                    "module": "C4",
                    "scenario": null
                },
                {
                    "value": "0,00E+00",
                    "module": "D",
                    "scenario": "S0"
                },
                {
                    "value": "0,00E+00",
                    "module": "D",
                    "scenario": "S1"
                },
                {
                    "value": "0,00E+00",
                    "module": "D",
                    "scenario": "S2"
                },
                {
                    "value": "0,00E+00",
                    "module": "D",
                    "scenario": "S3"
                }
            ]
        }
    ]
}