{
    "product_name": "Reinforcing stabilized three and seven-wire strands with and without dents with a nominal tensile strength of 1670\u00f71860 N /mm2 with a diameter of 6.5\u00f715.7 mm (PC-strand)",
    "epd_id": "EPD-Kiwa-EE-162692-EN",
    "declared_unit": {
        "unit": "kg",
        "amount": 1.0
    },
    "compliance": [
        "EN 15804+A2",
        "ISO 14025"
    ],
    "producer_name": "PJSC \"STALKANAT\"",
    "environmental_impact": [
        {
            "parameter": "GWP-total",
            "values": [
                {
                    "value": "2,54E+00",
                    "module": "A1",
                    "scenario": "Standard scenario"
                },
                {
                    "value": "2,27E-02",
                    "module": "A2",
                    "scenario": "Standard scenario"
                },
                {
                    "value": "2,71E-01",
                    "module": "A3",
                    "scenario": "Standard scenario"
                },
                {
                    "value": "0,00E+00",
                    "module": "C1",
                    "scenario": "Standard scenario"
                },
                {
                    "value": "7,09E-03",
                    "module": "C2",
                    "scenario": "Standard scenario"
                },
                {
                    "value": "0,00E+00",
                    "module": "C3",
                    "scenario": "Standard scenario"
                },
                {
                    "value": "2,64E-04",
                    "module": "C4",
                    "scenario": "Standard scenario"
                },
                {
                    "value": "-1,34E+00",
                    "module": "D",
                    "scenario": "Standard scenario"
                }
            ]
        },
        {
            "parameter": "GWP-fossil",
            "values": [
                {
                    "value": "2,54E+00",
                    "module": "A1",
                    "scenario": "Standard scenario"
                },
                {
                    "value": "2,25E-02",
                    "module": "A2",
                    "scenario": "Standard scenario"
                },
                {
                    "value": "2,60E-01",
                    "module": "A3",
                    "scenario": "Standard scenario"
                },
                {
                    "value": "0,00E+00",
                    "module": "C1",
                    "scenario": "Standard scenario"
                },
                {
                    "value": "7,09E-03",
                    "module": "C2",
                    "scenario": "Standard scenario"
                },
                {
                    "value": "0,00E+00",
                    "module": "C3",
                    "scenario": "Standard scenario"
                },
                {
                    "value": "2,63E-04",
                    "module": "C4",
                    "scenario": "Standard scenario"
                },
                {
                    "value": "-1,35E+00",
                    "module": "D",
                    "scenario": "Standard scenario"
                }
            ]
        },
        {
            "parameter": "GWP-biogenic",
            "values": [
                {
                    "value": "-3,12E-03",
                    "module": "A1",
                    "scenario": "Standard scenario"
                },
                {
                    "value": "1,29E-04",
                    "module": "A2",
                    "scenario": "Standard scenario"
                },
                {
                    "value": "2,83E-03",
                    "module": "A3",
                    "scenario": "Standard scenario"
                },
                {
                    "value": "0,00E+00",
                    "module": "C1",
                    "scenario": "Standard scenario"
                },
                {
                    "value": "3,27E-06",
                    "module": "C2",
                    "scenario": "Standard scenario"
                },
                {
                    "value": "0,00E+00",
                    "module": "C3",
                    "scenario": "Standard scenario"
                },
                {
                    "value": "5,22E-07",
                    "module": "C4",
                    "scenario": "Standard scenario"
                },
                {
                    "value": "1,41E-02",
                    "module": "D",
                    "scenario": "Standard scenario"
                }
            ]
        },
        {
            "parameter": "GWP-luluc",
            "values": [
                {
                    "value": "3,35E-04",
                    "module": "A1",
                    "scenario": "Standard scenario"
                },
                {
                    "value": "2,67E-05",
                    "module": "A2",
                    "scenario": "Standard scenario"
                },
                {
                    "value": "8,14E-03",
                    "module": "A3",
                    "scenario": "Standard scenario"
                },
                {
                    "value": "0,00E+00",
                    "module": "C1",
                    "scenario": "Standard scenario"
                },
                {
                    "value": "2,60E-06",
                    "module": "C2",
                    "scenario": "Standard scenario"
                },
                {
                    "value": "0,00E+00",
                    "module": "C3",
                    "scenario": "Standard scenario"
                },
                {
                    "value": "7,34E-08",
                    "module": "C4",
                    "scenario": "Standard scenario"
                },
                {
                    "value": "9,99E-04",
                    "module": "D",
                    "scenario": "Standard scenario"
                }
            ]
        },
        {
            "parameter": "ODP",
            "values": [
                {
                    "value": "2,00E-15",
                    "module": "A1",
                    "scenario": "Standard scenario"
                },
                {
                    "value": "3,08E-09",
                    "module": "A2",
                    "scenario": "Standard scenario"
                },
                {
                    "value": "8,18E-09",
                    "module": "A3",
                    "scenario": "Standard scenario"
                },
                {
                    "value": "0,00E+00",
                    "module": "C1",
                    "scenario": "Standard scenario"
                },
                {
                    "value": "1,56E-09",
                    "module": "C2",
                    "scenario": "Standard scenario"
                },
                {
                    "value": "0,00E+00",
                    "module": "C3",
                    "scenario": "Standard scenario"
                },
                {
                    "value": "1,08E-10",
                    "module": "C4",
                    "scenario": "Standard scenario"
                },
                {
                    "value": "-3,30E-08",
                    "module": "D",
                    "scenario": "Standard scenario"
                }
            ]
        },
        {
            "parameter": "AP",
            "values": [
                {
                    "value": "2,92E-03",
                    "module": "A1",
                    "scenario": "Standard scenario"
                },
                {
                    "value": "1,92E-04",
                    "module": "A2",
                    "scenario": "Standard scenario"
                },
                {
                    "value": "1,01E-03",
                    "module": "A3",
                    "scenario": "Standard scenario"
                },
                {
                    "value": "0,00E+00",
                    "module": "C1",
                    "scenario": "Standard scenario"
                },
                {
                    "value": "4,11E-05",
                    "module": "C2",
                    "scenario": "Standard scenario"
                },
                {
                    "value": "0,00E+00",
                    "module": "C3",
                    "scenario": "Standard scenario"
                },
                {
                    "value": "2,50E-06",
                    "module": "C4",
                    "scenario": "Standard scenario"
                },
                {
                    "value": "-5,22E-03",
                    "module": "D",
                    "scenario": "Standard scenario"
                }
            ]
        },
        {
            "parameter": "POCP",
            "values": [
                {
                    "value": "1,28E-07",
                    "module": "A1",
                    "scenario": "Standard scenario"
                },
                {
                    "value": "2,03E-04",
                    "module": "A2",
                    "scenario": "Standard scenario"
                },
                {
                    "value": "3,35E-04",
                    "module": "A3",
                    "scenario": "Standard scenario"
                },
                {
                    "value": "0,00E+00",
                    "module": "C1",
                    "scenario": "Standard scenario"
                },
                {
                    "value": "4,56E-05",
                    "module": "C2",
                    "scenario": "Standard scenario"
                },
                {
                    "value": "0,00E+00",
                    "module": "C3",
                    "scenario": "Standard scenario"
                },
                {
                    "value": "2,75E-06",
                    "module": "C4",
                    "scenario": "Standard scenario"
                },
                {
                    "value": "-7,69E-03",
                    "module": "D",
                    "scenario": "Standard scenario"
                }
            ]
        },
        {
            "parameter": "ADPE",
            "values": [
                {
                    "value": "2,60E+01",
                    "module": "A1",
                    "scenario": "Standard scenario"
                },
                {
                    "value": "1,81E-07",
                    "module": "A2",
                    "scenario": "Standard scenario"
                },
                {
                    "value": "6,97E-01",
                    "module": "A3",
                    "scenario": "Standard scenario"
                },
                {
                    "value": "0,00E+00",
                    "module": "C1",
                    "scenario": "Standard scenario"
                },
                {
                    "value": "1,80E-07",
                    "module": "C2",
                    "scenario": "Standard scenario"
                },
                {
                    "value": "0,00E+00",
                    "module": "C3",
                    "scenario": "Standard scenario"
                },
                {
                    "value": "2,41E-09",
                    "module": "C4",
                    "scenario": "Standard scenario"
                },
                {
                    "value": "-9,14E-07",
                    "module": "D",
                    "scenario": "Standard scenario"
                }
            ]
        },
        {
            "parameter": "ADPF",
            "values": [
                {
                    "value": "5,06E+00",
                    "module": "A1",
                    "scenario": "Standard scenario"
                },
                {
                    "value": "3,31E-01",
                    "module": "A2",
                    "scenario": "Standard scenario"
                },
                {
                    "value": "1,86E+00",
                    "module": "A3",
                    "scenario": "Standard scenario"
                },
                {
                    "value": "0,00E+00",
                    "module": "C1",
                    "scenario": "Standard scenario"
                },
                {
                    "value": "1,07E-01",
                    "module": "C2",
                    "scenario": "Standard scenario"
                },
                {
                    "value": "0,00E+00",
                    "module": "C3",
                    "scenario": "Standard scenario"
                },
                {
                    "value": "7,36E-03",
                    "module": "C4",
                    "scenario": "Standard scenario"
                },
                {
                    "value": "-9,45E+00",
                    "module": "D",
                    "scenario": "Standard scenario"
                }
            ]
        },
        {
            "parameter": "WDP",
            "values": [
                {
                    "value": "2,78E-08",
                    "module": "A1",
                    "scenario": "Standard scenario"
                },
                {
                    "value": "2,92E-03",
                    "module": "A2",
                    "scenario": "Standard scenario"
                },
                {
                    "value": "6,38E-01",
                    "module": "A3",
                    "scenario": "Standard scenario"
                },
                {
                    "value": "0,00E+00",
                    "module": "C1",
                    "scenario": "Standard scenario"
                },
                {
                    "value": "3,82E-04",
                    "module": "C2",
                    "scenario": "Standard scenario"
                },
                {
                    "value": "0,00E+00",
                    "module": "C3",
                    "scenario": "Standard scenario"
                },
                {
                    "value": "3,30E-04",
                    "module": "C4",
                    "scenario": "Standard scenario"
                },
                {
                    "value": "-2,58E-01",
                    "module": "D",
                    "scenario": "Standard scenario"
                }
            ]
        },
        {
            "parameter": "EP-freshwater",
            "values": [
                {
                    "value": "3,49E+00",
                    "module": "A1",
                    "scenario": "Standard scenario"
                },
                {
                    "value": "9,51E-07",
                    "module": "A2",
                    "scenario": "Standard scenario"
                },
                {
                    "value": "9,36E-02",
                    "module": "A3",
                    "scenario": "Standard scenario"
                },
                {
                    "value": "0,00E+00",
                    "module": "C1",
                    "scenario": "Standard scenario"
                },
                {
                    "value": "7,15E-08",
                    "module": "C2",
                    "scenario": "Standard scenario"
                },
                {
                    "value": "0,00E+00",
                    "module": "C3",
                    "scenario": "Standard scenario"
                },
                {
                    "value": "2,95E-09",
                    "module": "C4",
                    "scenario": "Standard scenario"
                },
                {
                    "value": "-4,78E-05",
                    "module": "D",
                    "scenario": "Standard scenario"
                }
            ]
        },
        {
            "parameter": "EP-marine",
            "values": [
                {
                    "value": "6,15E-03",
                    "module": "A1",
                    "scenario": "Standard scenario"
                },
                {
                    "value": "6,74E-05",
                    "module": "A2",
                    "scenario": "Standard scenario"
                },
                {
                    "value": "3,53E-04",
                    "module": "A3",
                    "scenario": "Standard scenario"
                },
                {
                    "value": "0,00E+00",
                    "module": "C1",
                    "scenario": "Standard scenario"
                },
                {
                    "value": "1,45E-05",
                    "module": "C2",
                    "scenario": "Standard scenario"
                },
                {
                    "value": "0,00E+00",
                    "module": "C3",
                    "scenario": "Standard scenario"
                },
                {
                    "value": "8,60E-07",
                    "module": "C4",
                    "scenario": "Standard scenario"
                },
                {
                    "value": "-9,68E-04",
                    "module": "D",
                    "scenario": "Standard scenario"
                }
            ]
        },
        {
            "parameter": "EP-terrestrial",
            "values": [
                {
                    "value": "1,65E-03",
                    "module": "A1",
                    "scenario": "Standard scenario"
                },
                {
                    "value": "7,47E-04",
                    "module": "A2",
                    "scenario": "Standard scenario"
                },
                {
                    "value": "1,62E-03",
                    "module": "A3",
                    "scenario": "Standard scenario"
                },
                {
                    "value": "0,00E+00",
                    "module": "C1",
                    "scenario": "Standard scenario"
                },
                {
                    "value": "1,60E-04",
                    "module": "C2",
                    "scenario": "Standard scenario"
                },
                {
                    "value": "0,00E+00",
                    "module": "C3",
                    "scenario": "Standard scenario"
                },
                {
                    "value": "9,48E-06",
                    "module": "C4",
                    "scenario": "Standard scenario"
                },
                {
                    "value": "-1,13E-02",
                    "module": "D",
                    "scenario": "Standard scenario"
                }
            ]
        }
    ],
    "additional_environmental_impact": [
        {
            "parameter": "PM",
            "values": [
                {
                    "value": "6,15E-03",
                    "module": "A1",
                    "scenario": "Standard scenario"
                },
                {
                    "value": "1,68E-09",
                    "module": "A2",
                    "scenario": "Standard scenario"
                },
                {
                    "value": "1,65E-04",
                    "module": "A3",
                    "scenario": "Standard scenario"
                },
                {
                    "value": "0,00E+00",
                    "module": "C1",
                    "scenario": "Standard scenario"
                },
                {
                    "value": "6,37E-10",
                    "module": "C2",
                    "scenario": "Standard scenario"
                },
                {
                    "value": "0,00E+00",
                    "module": "C3",
                    "scenario": "Standard scenario"
                },
                {
                    "value": "4,86E-11",
                    "module": "C4",
                    "scenario": "Standard scenario"
                },
                {
                    "value": "-7,83E-08",
                    "module": "D",
                    "scenario": "Standard scenario"
                }
            ]
        },
        {
            "parameter": "ETP-fw",
            "values": [
                {
                    "value": "3,49E+00",
                    "module": "A1",
                    "scenario": "Standard scenario"
                },
                {
                    "value": "3,54E-01",
                    "module": "A2",
                    "scenario": "Standard scenario"
                },
                {
                    "value": "3,23E+00",
                    "module": "A3",
                    "scenario": "Standard scenario"
                },
                {
                    "value": "0,00E+00",
                    "module": "C1",
                    "scenario": "Standard scenario"
                },
                {
                    "value": "9,53E-02",
                    "module": "C2",
                    "scenario": "Standard scenario"
                },
                {
                    "value": "0,00E+00",
                    "module": "C3",
                    "scenario": "Standard scenario"
                },
                {
                    "value": "4,77E-03",
                    "module": "C4",
                    "scenario": "Standard scenario"
                },
                {
                    "value": "-4,54E+01",
                    "module": "D",
                    "scenario": "Standard scenario"
                }
            ]
        },
        {
            "parameter": "HTP-c",
            "values": [
                {
                    "value": "1,23E-10",
                    "module": "A1",
                    "scenario": "Standard scenario"
                },
                {
                    "value": "2,16E-11",
                    "module": "A2",
                    "scenario": "Standard scenario"
                },
                {
                    "value": "1,03E-09",
                    "module": "A3",
                    "scenario": "Standard scenario"
                },
                {
                    "value": "0,00E+00",
                    "module": "C1",
                    "scenario": "Standard scenario"
                },
                {
                    "value": "3,09E-12",
                    "module": "C2",
                    "scenario": "Standard scenario"
                },
                {
                    "value": "0,00E+00",
                    "module": "C3",
                    "scenario": "Standard scenario"
                },
                {
                    "value": "1,10E-13",
                    "module": "C4",
                    "scenario": "Standard scenario"
                },
                {
                    "value": "-1,75E-10",
                    "module": "D",
                    "scenario": "Standard scenario"
                }
            ]
        },
        {
            "parameter": "HTP-nc",
            "values": [
                {
                    "value": "1,12E-08",
                    "module": "A1",
                    "scenario": "Standard scenario"
                },
                {
                    "value": "3,96E-10",
                    "module": "A2",
                    "scenario": "Standard scenario"
                },
                {
                    "value": "1,28E-08",
                    "module": "A3",
                    "scenario": "Standard scenario"
                },
                {
                    "value": "0,00E+00",
                    "module": "C1",
                    "scenario": "Standard scenario"
                },
                {
                    "value": "1,04E-10",
                    "module": "C2",
                    "scenario": "Standard scenario"
                },
                {
                    "value": "0,00E+00",
                    "module": "C3",
                    "scenario": "Standard scenario"
                },
                {
                    "value": "3,39E-12",
                    "module": "C4",
                    "scenario": "Standard scenario"
                },
                {
                    "value": "2,62E-07",
                    "module": "D",
                    "scenario": "Standard scenario"
                }
            ]
        },
        {
            "parameter": "SQP",
            "values": [
                {
                    "value": "1,64E+00",
                    "module": "A1",
                    "scenario": "Standard scenario"
                },
                {
                    "value": "2,28E-01",
                    "module": "A2",
                    "scenario": "Standard scenario"
                },
                {
                    "value": "8,33E-01",
                    "module": "A3",
                    "scenario": "Standard scenario"
                },
                {
                    "value": "0,00E+00",
                    "module": "C1",
                    "scenario": "Standard scenario"
                },
                {
                    "value": "9,27E-02",
                    "module": "C2",
                    "scenario": "Standard scenario"
                },
                {
                    "value": "0,00E+00",
                    "module": "C3",
                    "scenario": "Standard scenario"
                },
                {
                    "value": "1,54E-02",
                    "module": "C4",
                    "scenario": "Standard scenario"
                },
                {
                    "value": "-2,09E+00",
                    "module": "D",
                    "scenario": "Standard scenario"
                }
            ]
        },
        {
            "parameter": "IRP",
            "values": [
                {
                    "value": "5,22E-02",
                    "module": "A1",
                    "scenario": "Standard scenario"
                },
                {
                    "value": "1,85E-03",
                    "module": "A2",
                    "scenario": "Standard scenario"
                },
                {
                    "value": "1,62E-02",
                    "module": "A3",
                    "scenario": "Standard scenario"
                },
                {
                    "value": "0,00E+00",
                    "module": "C1",
                    "scenario": "Standard scenario"
                },
                {
                    "value": "4,48E-04",
                    "module": "C2",
                    "scenario": "Standard scenario"
                },
                {
                    "value": "0,00E+00",
                    "module": "C3",
                    "scenario": "Standard scenario"
                },
                {
                    "value": "3,02E-05",
                    "module": "C4",
                    "scenario": "Standard scenario"
                },
                {
                    "value": "2,31E-02",
                    "module": "D",
                    "scenario": "Standard scenario"
                }
            ]
        }
    ],
    "resource_use": [
        {
            "parameter": "PERE",
            "values": [
                {
                    "value": "4,94E-01",
                    "module": "A1",
                    "scenario": "Standard scenario"
                },
                {
                    "value": "2,85E-02",
                    "module": "A2",
                    "scenario": "Standard scenario"
                },
                {
                    "value": "1,63E-01",
                    "module": "A3",
                    "scenario": "Standard scenario"
                },
                {
                    "value": "0,00E+00",
                    "module": "C1",
                    "scenario": "Standard scenario"
                },
                {
                    "value": "1,34E-03",
                    "module": "C2",
                    "scenario": "Standard scenario"
                },
                {
                    "value": "0,00E+00",
                    "module": "C3",
                    "scenario": "Standard scenario"
                },
                {
                    "value": "5,95E-05",
                    "module": "C4",
                    "scenario": "Standard scenario"
                },
                {
                    "value": "2,75E-01",
                    "module": "D",
                    "scenario": "Standard scenario"
                }
            ]
        },
        {
            "parameter": "PERM",
            "values": [
                {
                    "value": "0,00E+00",
                    "module": "A1",
                    "scenario": "Standard scenario"
                },
                {
                    "value": "0,00E+00",
                    "module": "A2",
                    "scenario": "Standard scenario"
                },
                {
                    "value": "0,00E+00",
                    "module": "A3",
                    "scenario": "Standard scenario"
                },
                {
                    "value": "0,00E+00",
                    "module": "C1",
                    "scenario": "Standard scenario"
                },
                {
                    "value": "0,00E+00",
                    "module": "C2",
                    "scenario": "Standard scenario"
                },
                {
                    "value": "0,00E+00",
                    "module": "C3",
                    "scenario": "Standard scenario"
                },
                {
                    "value": "0,00E+00",
                    "module": "C4",
                    "scenario": "Standard scenario"
                },
                {
                    "value": "0,00E+00",
                    "module": "D",
                    "scenario": "Standard scenario"
                }
            ]
        },
        {
            "parameter": "PERT",
            "values": [
                {
                    "value": "4,94E-01",
                    "module": "A1",
                    "scenario": "Standard scenario"
                },
                {
                    "value": "2,85E-02",
                    "module": "A2",
                    "scenario": "Standard scenario"
                },
                {
                    "value": "1,63E-01",
                    "module": "A3",
                    "scenario": "Standard scenario"
                },
                {
                    "value": "0,00E+00",
                    "module": "C1",
                    "scenario": "Standard scenario"
                },
                {
                    "value": "1,34E-03",
                    "module": "C2",
                    "scenario": "Standard scenario"
                },
                {
                    "value": "0,00E+00",
                    "module": "C3",
                    "scenario": "Standard scenario"
                },
                {
                    "value": "5,95E-05",
                    "module": "C4",
                    "scenario": "Standard scenario"
                },
                {
                    "value": "2,75E-01",
                    "module": "D",
                    "scenario": "Standard scenario"
                }
            ]
        },
        {
            "parameter": "PENRE",
            "values": [
                {
                    "value": "2,60E+01",
                    "module": "A1",
                    "scenario": "Standard scenario"
                },
                {
                    "value": "3,50E-01",
                    "module": "A2",
                    "scenario": "Standard scenario"
                },
                {
                    "value": "2,44E+00",
                    "module": "A3",
                    "scenario": "Standard scenario"
                },
                {
                    "value": "0,00E+00",
                    "module": "C1",
                    "scenario": "Standard scenario"
                },
                {
                    "value": "1,13E-01",
                    "module": "C2",
                    "scenario": "Standard scenario"
                },
                {
                    "value": "0,00E+00",
                    "module": "C3",
                    "scenario": "Standard scenario"
                },
                {
                    "value": "7,82E-03",
                    "module": "C4",
                    "scenario": "Standard scenario"
                },
                {
                    "value": "-9,81E+00",
                    "module": "D",
                    "scenario": "Standard scenario"
                }
            ]
        },
        {
            "parameter": "PENRM",
            "values": [
                {
                    "value": "0,00E+00",
                    "module": "A1",
                    "scenario": "Standard scenario"
                },
                {
                    "value": "0,00E+00",
                    "module": "A2",
                    "scenario": "Standard scenario"
                },
                {
                    "value": "5,66E-02",
                    "module": "A3",
                    "scenario": "Standard scenario"
                },
                {
                    "value": "0,00E+00",
                    "module": "C1",
                    "scenario": "Standard scenario"
                },
                {
                    "value": "0,00E+00",
                    "module": "C2",
                    "scenario": "Standard scenario"
                },
                {
                    "value": "0,00E+00",
                    "module": "C3",
                    "scenario": "Standard scenario"
                },
                {
                    "value": "0,00E+00",
                    "module": "C4",
                    "scenario": "Standard scenario"
                },
                {
                    "value": "0,00E+00",
                    "module": "D",
                    "scenario": "Standard scenario"
                }
            ]
        },
        {
            "parameter": "PENRT",
            "values": [
                {
                    "value": "2,60E+01",
                    "module": "A1",
                    "scenario": "Standard scenario"
                },
                {
                    "value": "3,50E-01",
                    "module": "A2",
                    "scenario": "Standard scenario"
                },
                {
                    "value": "2,50E+00",
                    "module": "A3",
                    "scenario": "Standard scenario"
                },
                {
                    "value": "0,00E+00",
                    "module": "C1",
                    "scenario": "Standard scenario"
                },
                {
                    "value": "1,13E-01",
                    "module": "C2",
                    "scenario": "Standard scenario"
                },
                {
                    "value": "0,00E+00",
                    "module": "C3",
                    "scenario": "Standard scenario"
                },
                {
                    "value": "7,82E-03",
                    "module": "C4",
                    "scenario": "Standard scenario"
                },
                {
                    "value": "-9,81E+00",
                    "module": "D",
                    "scenario": "Standard scenario"
                }
            ]
        },
        {
            "parameter": "SM",
            "values": [
                {
                    "value": "1,67E-01",
                    "module": "A1",
                    "scenario": "Standard scenario"
                },
                {
                    "value": "0,00E+00",
                    "module": "A2",
                    "scenario": "Standard scenario"
                },
                {
                    "value": "5,16E-03",
                    "module": "A3",
                    "scenario": "Standard scenario"
                },
                {
                    "value": "0,00E+00",
                    "module": "C1",
                    "scenario": "Standard scenario"
                },
                {
                    "value": "0,00E+00",
                    "module": "C2",
                    "scenario": "Standard scenario"
                },
                {
                    "value": "0,00E+00",
                    "module": "C3",
                    "scenario": "Standard scenario"
                },
                {
                    "value": "0,00E+00",
                    "module": "C4",
                    "scenario": "Standard scenario"
                },
                {
                    "value": "0,00E+00",
                    "module": "D",
                    "scenario": "Standard scenario"
                }
            ]
        },
        {
            "parameter": "RSF",
            "values": [
                {
                    "value": "0,00E+00",
                    "module": "A1",
                    "scenario": "Standard scenario"
                },
                {
                    "value": "0,00E+00",
                    "module": "A2",
                    "scenario": "Standard scenario"
                },
                {
                    "value": "0,00E+00",
                    "module": "A3",
                    "scenario": "Standard scenario"
                },
                {
                    "value": "0,00E+00",
                    "module": "C1",
                    "scenario": "Standard scenario"
                },
                {
                    "value": "0,00E+00",
                    "module": "C2",
                    "scenario": "Standard scenario"
                },
                {
                    "value": "0,00E+00",
                    "module": "C3",
                    "scenario": "Standard scenario"
                },
                {
                    "value": "0,00E+00",
                    "module": "C4",
                    "scenario": "Standard scenario"
                },
                {
                    "value": "0,00E+00",
                    "module": "D",
                    "scenario": "Standard scenario"
                }
            ]
        },
        {
            "parameter": "NRSF",
            "values": [
                {
                    "value": "0,00E+00",
                    "module": "A1",
                    "scenario": "Standard scenario"
                },
                {
                    "value": "0,00E+00",
                    "module": "A2",
                    "scenario": "Standard scenario"
                },
                {
                    "value": "0,00E+00",
                    "module": "A3",
                    "scenario": "Standard scenario"
                },
                {
                    "value": "0,00E+00",
                    "module": "C1",
                    "scenario": "Standard scenario"
                },
                {
                    "value": "0,00E+00",
                    "module": "C2",
                    "scenario": "Standard scenario"
                },
                {
                    "value": "0,00E+00",
                    "module": "C3",
                    "scenario": "Standard scenario"
                },
                {
                    "value": "0,00E+00",
                    "module": "C4",
                    "scenario": "Standard scenario"
                },
                {
                    "value": "0,00E+00",
                    "module": "D",
                    "scenario": "Standard scenario"
                }
            ]
        },
        {
            "parameter": "FW",
            "values": [
                {
                    "value": "1,19E-01",
                    "module": "A1",
                    "scenario": "Standard scenario"
                },
                {
                    "value": "1,55E-04",
                    "module": "A2",
                    "scenario": "Standard scenario"
                },
                {
                    "value": "1,84E-02",
                    "module": "A3",
                    "scenario": "Standard scenario"
                },
                {
                    "value": "0,00E+00",
                    "module": "C1",
                    "scenario": "Standard scenario"
                },
                {
                    "value": "1,30E-05",
                    "module": "C2",
                    "scenario": "Standard scenario"
                },
                {
                    "value": "0,00E+00",
                    "module": "C3",
                    "scenario": "Standard scenario"
                },
                {
                    "value": "7,86E-06",
                    "module": "C4",
                    "scenario": "Standard scenario"
                },
                {
                    "value": "-4,89E-03",
                    "module": "D",
                    "scenario": "Standard scenario"
                }
            ]
        }
    ],
    "end_of_life_waste": [
        {
            "parameter": "HWD",
            "values": [
                {
                    "value": "1,92E-09",
                    "module": "A1",
                    "scenario": "Standard scenario"
                },
                {
                    "value": "6,42E-07",
                    "module": "A2",
                    "scenario": "Standard scenario"
                },
                {
                    "value": "4,27E-06",
                    "module": "A3",
                    "scenario": "Standard scenario"
                },
                {
                    "value": "0,00E+00",
                    "module": "C1",
                    "scenario": "Standard scenario"
                },
                {
                    "value": "2,71E-07",
                    "module": "C2",
                    "scenario": "Standard scenario"
                },
                {
                    "value": "0,00E+00",
                    "module": "C3",
                    "scenario": "Standard scenario"
                },
                {
                    "value": "1,10E-08",
                    "module": "C4",
                    "scenario": "Standard scenario"
                },
                {
                    "value": "-1,62E-04",
                    "module": "D",
                    "scenario": "Standard scenario"
                }
            ]
        },
        {
            "parameter": "NHWD",
            "values": [
                {
                    "value": "2,36E-01",
                    "module": "A1",
                    "scenario": "Standard scenario"
                },
                {
                    "value": "4,46E-03",
                    "module": "A2",
                    "scenario": "Standard scenario"
                },
                {
                    "value": "1,01E-01",
                    "module": "A3",
                    "scenario": "Standard scenario"
                },
                {
                    "value": "0,00E+00",
                    "module": "C1",
                    "scenario": "Standard scenario"
                },
                {
                    "value": "6,78E-03",
                    "module": "C2",
                    "scenario": "Standard scenario"
                },
                {
                    "value": "0,00E+00",
                    "module": "C3",
                    "scenario": "Standard scenario"
                },
                {
                    "value": "5,00E-02",
                    "module": "C4",
                    "scenario": "Standard scenario"
                },
                {
                    "value": "-1,32E-01",
                    "module": "D",
                    "scenario": "Standard scenario"
                }
            ]
        },
        {
            "parameter": "RWD",
            "values": [
                {
                    "value": "6,56E-04",
                    "module": "A1",
                    "scenario": "Standard scenario"
                },
                {
                    "value": "2,03E-06",
                    "module": "A2",
                    "scenario": "Standard scenario"
                },
                {
                    "value": "3,01E-05",
                    "module": "A3",
                    "scenario": "Standard scenario"
                },
                {
                    "value": "0,00E+00",
                    "module": "C1",
                    "scenario": "Standard scenario"
                },
                {
                    "value": "7,02E-07",
                    "module": "C2",
                    "scenario": "Standard scenario"
                },
                {
                    "value": "0,00E+00",
                    "module": "C3",
                    "scenario": "Standard scenario"
                },
                {
                    "value": "4,83E-08",
                    "module": "C4",
                    "scenario": "Standard scenario"
                },
                {
                    "value": "8,01E-06",
                    "module": "D",
                    "scenario": "Standard scenario"
                }
            ]
        }
    ],
    "end_of_life_flow": [
        {
            "parameter": "CRU",
            "values": [
                {
                    "value": "0,00E+00",
                    "module": "A1",
                    "scenario": "Standard scenario"
                },
                {
                    "value": "0,00E+00",
                    "module": "A2",
                    "scenario": "Standard scenario"
                },
                {
                    "value": "0,00E+00",
                    "module": "A3",
                    "scenario": "Standard scenario"
                },
                {
                    "value": "0,00E+00",
                    "module": "C1",
                    "scenario": "Standard scenario"
                },
                {
                    "value": "0,00E+00",
                    "module": "C2",
                    "scenario": "Standard scenario"
                },
                {
                    "value": "0,00E+00",
                    "module": "C3",
                    "scenario": "Standard scenario"
                },
                {
                    "value": "0,00E+00",
                    "module": "C4",
                    "scenario": "Standard scenario"
                },
                {
                    "value": "0,00E+00",
                    "module": "D",
                    "scenario": "Standard scenario"
                }
            ]
        },
        {
            "parameter": "MFR",
            "values": [
                {
                    "value": "4,52E-04",
                    "module": "A1",
                    "scenario": "Standard scenario"
                },
                {
                    "value": "0,00E+00",
                    "module": "A2",
                    "scenario": "Standard scenario"
                },
                {
                    "value": "2,55E-02",
                    "module": "A3",
                    "scenario": "Standard scenario"
                },
                {
                    "value": "0,00E+00",
                    "module": "C1",
                    "scenario": "Standard scenario"
                },
                {
                    "value": "0,00E+00",
                    "module": "C2",
                    "scenario": "Standard scenario"
                },
                {
                    "value": "9,50E-01",
                    "module": "C3",
                    "scenario": "Standard scenario"
                },
                {
                    "value": "0,00E+00",
                    "module": "C4",
                    "scenario": "Standard scenario"
                },
                {
                    "value": "0,00E+00",
                    "module": "D",
                    "scenario": "Standard scenario"
                }
            ]
        },
        {
            "parameter": "MER",
            "values": [
                {
                    "value": "0,00E+00",
                    "module": "A1",
                    "scenario": "Standard scenario"
                },
                {
                    "value": "0,00E+00",
                    "module": "A2",
                    "scenario": "Standard scenario"
                },
                {
                    "value": "0,00E+00",
                    "module": "A3",
                    "scenario": "Standard scenario"
                },
                {
                    "value": "0,00E+00",
                    "module": "C1",
                    "scenario": "Standard scenario"
                },
                {
                    "value": "0,00E+00",
                    "module": "C2",
                    "scenario": "Standard scenario"
                },
                {
                    "value": "0,00E+00",
                    "module": "C3",
                    "scenario": "Standard scenario"
                },
                {
                    "value": "0,00E+00",
                    "module": "C4",
                    "scenario": "Standard scenario"
                },
                {
                    "value": "0,00E+00",
                    "module": "D",
                    "scenario": "Standard scenario"
                }
            ]
        },
        {
            "parameter": "EEE",
            "values": [
                {
                    "value": "0,00E+00",
                    "module": "A1",
                    "scenario": "Standard scenario"
                },
                {
                    "value": "0,00E+00",
                    "module": "A2",
                    "scenario": "Standard scenario"
                },
                {
                    "value": "8,12E-03",
                    "module": "A3",
                    "scenario": "Standard scenario"
                },
                {
                    "value": "0,00E+00",
                    "module": "C1",
                    "scenario": "Standard scenario"
                },
                {
                    "value": "0,00E+00",
                    "module": "C2",
                    "scenario": "Standard scenario"
                },
                {
                    "value": "0,00E+00",
                    "module": "C3",
                    "scenario": "Standard scenario"
                },
                {
                    "value": "0,00E+00",
                    "module": "C4",
                    "scenario": "Standard scenario"
                },
                {
                    "value": "0,00E+00",
                    "module": "D",
                    "scenario": "Standard scenario"
                }
            ]
        },
        {
            "parameter": "EET",
            "values": [
                {
                    "value": "0,00E+00",
                    "module": "A1",
                    "scenario": "Standard scenario"
                },
                {
                    "value": "0,00E+00",
                    "module": "A2",
                    "scenario": "Standard scenario"
                },
                {
                    "value": "1,40E-02",
                    "module": "A3",
                    "scenario": "Standard scenario"
                },
                {
                    "value": "0,00E+00",
                    "module": "C1",
                    "scenario": "Standard scenario"
                },
                {
                    "value": "0,00E+00",
                    "module": "C2",
                    "scenario": "Standard scenario"
                },
                {
                    "value": "0,00E+00",
                    "module": "C3",
                    "scenario": "Standard scenario"
                },
                {
                    "value": "0,00E+00",
                    "module": "C4",
                    "scenario": "Standard scenario"
                },
                {
                    "value": "0,00E+00",
                    "module": "D",
                    "scenario": "Standard scenario"
                }
            ]
        }
    ]
}