{
    "product_name": "Component EPD Ringebu: Extruded PE pipe systems from Ringebu - used as material component in various finished mixed products",
    "epd_id": "NEPD-7075-6470",
    "declared_unit": {
        "unit": "kg",
        "amount": 1.0
    },
    "compliance": [
        "EN 15804+A2",
        "ISO 14025",
        "ISO 21930"
    ],
    "producer_name": "Pipelife Norge AS",
    "environmental_impact": [
        {
            "parameter": "GWP-total",
            "values": [
                {
                    "value": "2,03E+00",
                    "module": "A1-A3",
                    "scenario": null
                },
                {
                    "value": "1,63E-02",
                    "module": "A4",
                    "scenario": null
                },
                {
                    "value": "7,94E-02",
                    "module": "A5",
                    "scenario": null
                },
                {
                    "value": "0,00E+00",
                    "module": "C1",
                    "scenario": null
                },
                {
                    "value": "0,00E+00",
                    "module": "C2",
                    "scenario": null
                },
                {
                    "value": "1,40E+00",
                    "module": "C3",
                    "scenario": null
                },
                {
                    "value": "5,40E-02",
                    "module": "C4",
                    "scenario": null
                },
                {
                    "value": "-8,19E-02",
                    "module": "D",
                    "scenario": null
                }
            ]
        },
        {
            "parameter": "GWP-fossil",
            "values": [
                {
                    "value": "2,09E+00",
                    "module": "A1-A3",
                    "scenario": null
                },
                {
                    "value": "1,63E-02",
                    "module": "A4",
                    "scenario": null
                },
                {
                    "value": "3,21E-03",
                    "module": "A5",
                    "scenario": null
                },
                {
                    "value": "0,00E+00",
                    "module": "C1",
                    "scenario": null
                },
                {
                    "value": "0,00E+00",
                    "module": "C2",
                    "scenario": null
                },
                {
                    "value": "1,40E+00",
                    "module": "C3",
                    "scenario": null
                },
                {
                    "value": "5,40E-02",
                    "module": "C4",
                    "scenario": null
                },
                {
                    "value": "-7,90E-02",
                    "module": "D",
                    "scenario": null
                }
            ]
        },
        {
            "parameter": "GWP-biogenic",
            "values": [
                {
                    "value": "-6,38E-02",
                    "module": "A1-A3",
                    "scenario": null
                },
                {
                    "value": "6,76E-06",
                    "module": "A4",
                    "scenario": null
                },
                {
                    "value": "7,62E-02",
                    "module": "A5",
                    "scenario": null
                },
                {
                    "value": "0,00E+00",
                    "module": "C1",
                    "scenario": null
                },
                {
                    "value": "0,00E+00",
                    "module": "C2",
                    "scenario": null
                },
                {
                    "value": "1,13E-05",
                    "module": "C3",
                    "scenario": null
                },
                {
                    "value": "5,21E-06",
                    "module": "C4",
                    "scenario": null
                },
                {
                    "value": "-1,63E-04",
                    "module": "D",
                    "scenario": null
                }
            ]
        },
        {
            "parameter": "GWP-luluc",
            "values": [
                {
                    "value": "1,09E-03",
                    "module": "A1-A3",
                    "scenario": null
                },
                {
                    "value": "5,81E-06",
                    "module": "A4",
                    "scenario": null
                },
                {
                    "value": "8,82E-07",
                    "module": "A5",
                    "scenario": null
                },
                {
                    "value": "0,00E+00",
                    "module": "C1",
                    "scenario": null
                },
                {
                    "value": "0,00E+00",
                    "module": "C2",
                    "scenario": null
                },
                {
                    "value": "1,66E-06",
                    "module": "C3",
                    "scenario": null
                },
                {
                    "value": "1,17E-06",
                    "module": "C4",
                    "scenario": null
                },
                {
                    "value": "-2,72E-03",
                    "module": "D",
                    "scenario": null
                }
            ]
        },
        {
            "parameter": "ODP",
            "values": [
                {
                    "value": "7,41E-08",
                    "module": "A1-A3",
                    "scenario": null
                },
                {
                    "value": "3,70E-09",
                    "module": "A4",
                    "scenario": null
                },
                {
                    "value": "3,36E-10",
                    "module": "A5",
                    "scenario": null
                },
                {
                    "value": "0,00E+00",
                    "module": "C1",
                    "scenario": null
                },
                {
                    "value": "0,00E+00",
                    "module": "C2",
                    "scenario": null
                },
                {
                    "value": "1,07E-09",
                    "module": "C3",
                    "scenario": null
                },
                {
                    "value": "1,54E-09",
                    "module": "C4",
                    "scenario": null
                },
                {
                    "value": "-5,76E-03",
                    "module": "D",
                    "scenario": null
                }
            ]
        },
        {
            "parameter": "AP",
            "values": [
                {
                    "value": "8,12E-03",
                    "module": "A1-A3",
                    "scenario": null
                },
                {
                    "value": "4,69E-05",
                    "module": "A4",
                    "scenario": null
                },
                {
                    "value": "1,33E-05",
                    "module": "A5",
                    "scenario": null
                },
                {
                    "value": "0,00E+00",
                    "module": "C1",
                    "scenario": null
                },
                {
                    "value": "0,00E+00",
                    "module": "C2",
                    "scenario": null
                },
                {
                    "value": "1,75E-04",
                    "module": "C3",
                    "scenario": null
                },
                {
                    "value": "3,91E-05",
                    "module": "C4",
                    "scenario": null
                },
                {
                    "value": "-6,51E-04",
                    "module": "D",
                    "scenario": null
                }
            ]
        },
        {
            "parameter": "POCP",
            "values": [
                {
                    "value": "7,39E-03",
                    "module": "A1-A3",
                    "scenario": null
                },
                {
                    "value": "3,98E-05",
                    "module": "A4",
                    "scenario": null
                },
                {
                    "value": "1,55E-05",
                    "module": "A5",
                    "scenario": null
                },
                {
                    "value": "0,00E+00",
                    "module": "C1",
                    "scenario": null
                },
                {
                    "value": "0,00E+00",
                    "module": "C2",
                    "scenario": null
                },
                {
                    "value": "2,18E-04",
                    "module": "C3",
                    "scenario": null
                },
                {
                    "value": "5,51E-05",
                    "module": "C4",
                    "scenario": null
                },
                {
                    "value": "-6,35E-04",
                    "module": "D",
                    "scenario": null
                }
            ]
        },
        {
            "parameter": "ADPE",
            "values": [
                {
                    "value": "2,31E-05",
                    "module": "A1-A3",
                    "scenario": null
                },
                {
                    "value": "4,51E-07",
                    "module": "A4",
                    "scenario": null
                },
                {
                    "value": "3,15E-08",
                    "module": "A5",
                    "scenario": null
                },
                {
                    "value": "0,00E+00",
                    "module": "C1",
                    "scenario": null
                },
                {
                    "value": "0,00E+00",
                    "module": "C2",
                    "scenario": null
                },
                {
                    "value": "4,91E-08",
                    "module": "C3",
                    "scenario": null
                },
                {
                    "value": "4,01E-08",
                    "module": "C4",
                    "scenario": null
                },
                {
                    "value": "-7,86E-07",
                    "module": "D",
                    "scenario": null
                }
            ]
        },
        {
            "parameter": "ADPF",
            "values": [
                {
                    "value": "6,97E+01",
                    "module": "A1-A3",
                    "scenario": null
                },
                {
                    "value": "2,47E-01",
                    "module": "A4",
                    "scenario": null
                },
                {
                    "value": "2,38E-02",
                    "module": "A5",
                    "scenario": null
                },
                {
                    "value": "0,00E+00",
                    "module": "C1",
                    "scenario": null
                },
                {
                    "value": "0,00E+00",
                    "module": "C2",
                    "scenario": null
                },
                {
                    "value": "9,17E-02",
                    "module": "C3",
                    "scenario": null
                },
                {
                    "value": "1,15E-01",
                    "module": "C4",
                    "scenario": null
                },
                {
                    "value": "-1,13E+00",
                    "module": "D",
                    "scenario": null
                }
            ]
        },
        {
            "parameter": "WDP",
            "values": [
                {
                    "value": "2,04E+02",
                    "module": "A1-A3",
                    "scenario": null
                },
                {
                    "value": "2,39E-01",
                    "module": "A4",
                    "scenario": null
                },
                {
                    "value": "5,21E-02",
                    "module": "A5",
                    "scenario": null
                },
                {
                    "value": "0,00E+00",
                    "module": "C1",
                    "scenario": null
                },
                {
                    "value": "0,00E+00",
                    "module": "C2",
                    "scenario": null
                },
                {
                    "value": "2,08E-01",
                    "module": "C3",
                    "scenario": null
                },
                {
                    "value": "9,86E-01",
                    "module": "C4",
                    "scenario": null
                },
                {
                    "value": "-1,41E+01",
                    "module": "D",
                    "scenario": null
                }
            ]
        },
        {
            "parameter": "EP-freshwater",
            "values": [
                {
                    "value": "3,97E-05",
                    "module": "A1-A3",
                    "scenario": null
                },
                {
                    "value": "1,31E-07",
                    "module": "A4",
                    "scenario": null
                },
                {
                    "value": "2,58E-08",
                    "module": "A5",
                    "scenario": null
                },
                {
                    "value": "0,00E+00",
                    "module": "C1",
                    "scenario": null
                },
                {
                    "value": "0,00E+00",
                    "module": "C2",
                    "scenario": null
                },
                {
                    "value": "1,07E-07",
                    "module": "C3",
                    "scenario": null
                },
                {
                    "value": "5,99E-08",
                    "module": "C4",
                    "scenario": null
                },
                {
                    "value": "-7,02E-06",
                    "module": "D",
                    "scenario": null
                }
            ]
        },
        {
            "parameter": "EP-marine",
            "values": [
                {
                    "value": "1,47E-03",
                    "module": "A1-A3",
                    "scenario": null
                },
                {
                    "value": "9,29E-06",
                    "module": "A4",
                    "scenario": null
                },
                {
                    "value": "6,58E-06",
                    "module": "A5",
                    "scenario": null
                },
                {
                    "value": "0,00E+00",
                    "module": "C1",
                    "scenario": null
                },
                {
                    "value": "0,00E+00",
                    "module": "C2",
                    "scenario": null
                },
                {
                    "value": "8,42E-05",
                    "module": "C3",
                    "scenario": null
                },
                {
                    "value": "6,90E-05",
                    "module": "C4",
                    "scenario": null
                },
                {
                    "value": "-2,13E-04",
                    "module": "D",
                    "scenario": null
                }
            ]
        },
        {
            "parameter": "EP-terrestrial",
            "values": [
                {
                    "value": "1,64E-02",
                    "module": "A1-A3",
                    "scenario": null
                },
                {
                    "value": "1,04E-04",
                    "module": "A4",
                    "scenario": null
                },
                {
                    "value": "5,80E-05",
                    "module": "A5",
                    "scenario": null
                },
                {
                    "value": "0,00E+00",
                    "module": "C1",
                    "scenario": null
                },
                {
                    "value": "0,00E+00",
                    "module": "C2",
                    "scenario": null
                },
                {
                    "value": "9,11E-04",
                    "module": "C3",
                    "scenario": null
                },
                {
                    "value": "1,54E-04",
                    "module": "C4",
                    "scenario": null
                },
                {
                    "value": "-2,30E-03",
                    "module": "D",
                    "scenario": null
                }
            ]
        }
    ],
    "additional_environmental_impact": [
        {
            "parameter": "PM",
            "values": [
                {
                    "value": "7,12E-08",
                    "module": "A1-A3",
                    "scenario": null
                },
                {
                    "value": "1,00E-09",
                    "module": "A4",
                    "scenario": null
                },
                {
                    "value": "1,76E-10",
                    "module": "A5",
                    "scenario": null
                },
                {
                    "value": "0,00E+00",
                    "module": "C1",
                    "scenario": null
                },
                {
                    "value": "0,00E+00",
                    "module": "C2",
                    "scenario": null
                },
                {
                    "value": "6,88E-10",
                    "module": "C3",
                    "scenario": null
                },
                {
                    "value": "7,66E-10",
                    "module": "C4",
                    "scenario": null
                },
                {
                    "value": "-3,94E-08",
                    "module": "D",
                    "scenario": null
                }
            ]
        },
        {
            "parameter": "ETP-fw",
            "values": [
                {
                    "value": "1,54E+01",
                    "module": "A1-A3",
                    "scenario": null
                },
                {
                    "value": "1,83E-01",
                    "module": "A4",
                    "scenario": null
                },
                {
                    "value": "2,94E-02",
                    "module": "A5",
                    "scenario": null
                },
                {
                    "value": "0,00E+00",
                    "module": "C1",
                    "scenario": null
                },
                {
                    "value": "0,00E+00",
                    "module": "C2",
                    "scenario": null
                },
                {
                    "value": "2,74E-01",
                    "module": "C3",
                    "scenario": null
                },
                {
                    "value": "1,43E-01",
                    "module": "C4",
                    "scenario": null
                },
                {
                    "value": "-6,15E+00",
                    "module": "D",
                    "scenario": null
                }
            ]
        },
        {
            "parameter": "HTP-c",
            "values": [
                {
                    "value": "7,05E-10",
                    "module": "A1-A3",
                    "scenario": null
                },
                {
                    "value": "0,00E+00",
                    "module": "A4",
                    "scenario": null
                },
                {
                    "value": "2,00E-12",
                    "module": "A5",
                    "scenario": null
                },
                {
                    "value": "0,00E+00",
                    "module": "C1",
                    "scenario": null
                },
                {
                    "value": "0,00E+00",
                    "module": "C2",
                    "scenario": null
                },
                {
                    "value": "3,10E-11",
                    "module": "C3",
                    "scenario": null
                },
                {
                    "value": "4,00E-12",
                    "module": "C4",
                    "scenario": null
                },
                {
                    "value": "-1,12E-10",
                    "module": "D",
                    "scenario": null
                }
            ]
        },
        {
            "parameter": "HTP-nc",
            "values": [
                {
                    "value": "1,69E-08",
                    "module": "A1-A3",
                    "scenario": null
                },
                {
                    "value": "2,00E-10",
                    "module": "A4",
                    "scenario": null
                },
                {
                    "value": "1,05E-10",
                    "module": "A5",
                    "scenario": null
                },
                {
                    "value": "0,00E+00",
                    "module": "C1",
                    "scenario": null
                },
                {
                    "value": "0,00E+00",
                    "module": "C2",
                    "scenario": null
                },
                {
                    "value": "1,17E-09",
                    "module": "C3",
                    "scenario": null
                },
                {
                    "value": "1,10E-10",
                    "module": "C4",
                    "scenario": null
                },
                {
                    "value": "-5,89E-09",
                    "module": "D",
                    "scenario": null
                }
            ]
        },
        {
            "parameter": "SQP",
            "values": [
                {
                    "value": "6,71E+00",
                    "module": "A1-A3",
                    "scenario": null
                },
                {
                    "value": "1,73E-01",
                    "module": "A4",
                    "scenario": null
                },
                {
                    "value": "2,22E-02",
                    "module": "A5",
                    "scenario": null
                },
                {
                    "value": "0,00E+00",
                    "module": "C1",
                    "scenario": null
                },
                {
                    "value": "0,00E+00",
                    "module": "C2",
                    "scenario": null
                },
                {
                    "value": "1,11E-02",
                    "module": "C3",
                    "scenario": null
                },
                {
                    "value": "4,26E-01",
                    "module": "C4",
                    "scenario": null
                },
                {
                    "value": "-7,56E+00",
                    "module": "D",
                    "scenario": null
                }
            ]
        },
        {
            "parameter": "IRP",
            "values": [
                {
                    "value": "6,56E-02",
                    "module": "A1-A3",
                    "scenario": null
                },
                {
                    "value": "1,08E-03",
                    "module": "A4",
                    "scenario": null
                },
                {
                    "value": "9,23E-05",
                    "module": "A5",
                    "scenario": null
                },
                {
                    "value": "0,00E+00",
                    "module": "C1",
                    "scenario": null
                },
                {
                    "value": "0,00E+00",
                    "module": "C2",
                    "scenario": null
                },
                {
                    "value": "1,55E-04",
                    "module": "C3",
                    "scenario": null
                },
                {
                    "value": "5,54E-04",
                    "module": "C4",
                    "scenario": null
                },
                {
                    "value": "-7,22E-03",
                    "module": "D",
                    "scenario": null
                }
            ]
        }
    ],
    "resource_use": [
        {
            "parameter": "PERE",
            "values": [
                {
                    "value": "1,17E+01",
                    "module": "A1-A3",
                    "scenario": null
                },
                {
                    "value": "3,54E-03",
                    "module": "A4",
                    "scenario": null
                },
                {
                    "value": "7,96E-04",
                    "module": "A5",
                    "scenario": null
                },
                {
                    "value": "0,00E+00",
                    "module": "C1",
                    "scenario": null
                },
                {
                    "value": "0,00E+00",
                    "module": "C2",
                    "scenario": null
                },
                {
                    "value": "2,69E-03",
                    "module": "C3",
                    "scenario": null
                },
                {
                    "value": "5,41E-03",
                    "module": "C4",
                    "scenario": null
                },
                {
                    "value": "-6,98E+00",
                    "module": "D",
                    "scenario": null
                }
            ]
        },
        {
            "parameter": "PERM",
            "values": [
                {
                    "value": "6,98E-01",
                    "module": "A1-A3",
                    "scenario": null
                },
                {
                    "value": "0,00E+00",
                    "module": "A4",
                    "scenario": null
                },
                {
                    "value": "-6,98E-01",
                    "module": "A5",
                    "scenario": null
                },
                {
                    "value": "0,00E+00",
                    "module": "C1",
                    "scenario": null
                },
                {
                    "value": "0,00E+00",
                    "module": "C2",
                    "scenario": null
                },
                {
                    "value": "0,00E+00",
                    "module": "C3",
                    "scenario": null
                },
                {
                    "value": "0,00E+00",
                    "module": "C4",
                    "scenario": null
                },
                {
                    "value": "0,00E+00",
                    "module": "D",
                    "scenario": null
                }
            ]
        },
        {
            "parameter": "PERT",
            "values": [
                {
                    "value": "1,24E+01",
                    "module": "A1-A3",
                    "scenario": null
                },
                {
                    "value": "3,54E-03",
                    "module": "A4",
                    "scenario": null
                },
                {
                    "value": "-6,97E-01",
                    "module": "A5",
                    "scenario": null
                },
                {
                    "value": "0,00E+00",
                    "module": "C1",
                    "scenario": null
                },
                {
                    "value": "0,00E+00",
                    "module": "C2",
                    "scenario": null
                },
                {
                    "value": "2,69E-03",
                    "module": "C3",
                    "scenario": null
                },
                {
                    "value": "5,41E-03",
                    "module": "C4",
                    "scenario": null
                },
                {
                    "value": "-6,98E+00",
                    "module": "D",
                    "scenario": null
                }
            ]
        },
        {
            "parameter": "PENRE",
            "values": [
                {
                    "value": "3,22E+01",
                    "module": "A1-A3",
                    "scenario": null
                },
                {
                    "value": "2,47E-01",
                    "module": "A4",
                    "scenario": null
                },
                {
                    "value": "2,38E-02",
                    "module": "A5",
                    "scenario": null
                },
                {
                    "value": "0,00E+00",
                    "module": "C1",
                    "scenario": null
                },
                {
                    "value": "0,00E+00",
                    "module": "C2",
                    "scenario": null
                },
                {
                    "value": "9,17E-02",
                    "module": "C3",
                    "scenario": null
                },
                {
                    "value": "1,15E-01",
                    "module": "C4",
                    "scenario": null
                },
                {
                    "value": "-1,13E+00",
                    "module": "D",
                    "scenario": null
                }
            ]
        },
        {
            "parameter": "PENRM",
            "values": [
                {
                    "value": "4,03E+01",
                    "module": "A1-A3",
                    "scenario": null
                },
                {
                    "value": "0,00E+00",
                    "module": "A4",
                    "scenario": null
                },
                {
                    "value": "-8,76E-01",
                    "module": "A5",
                    "scenario": null
                },
                {
                    "value": "0,00E+00",
                    "module": "C1",
                    "scenario": null
                },
                {
                    "value": "0,00E+00",
                    "module": "C2",
                    "scenario": null
                },
                {
                    "value": "0,00E+00",
                    "module": "C3",
                    "scenario": null
                },
                {
                    "value": "0,00E+00",
                    "module": "C4",
                    "scenario": null
                },
                {
                    "value": "0,00E+00",
                    "module": "D",
                    "scenario": null
                }
            ]
        },
        {
            "parameter": "PENRT",
            "values": [
                {
                    "value": "7,25E+01",
                    "module": "A1-A3",
                    "scenario": null
                },
                {
                    "value": "2,47E-01",
                    "module": "A4",
                    "scenario": null
                },
                {
                    "value": "-8,52E-01",
                    "module": "A5",
                    "scenario": null
                },
                {
                    "value": "0,00E+00",
                    "module": "C1",
                    "scenario": null
                },
                {
                    "value": "0,00E+00",
                    "module": "C2",
                    "scenario": null
                },
                {
                    "value": "9,17E-02",
                    "module": "C3",
                    "scenario": null
                },
                {
                    "value": "1,15E-01",
                    "module": "C4",
                    "scenario": null
                },
                {
                    "value": "-1,13E+00",
                    "module": "D",
                    "scenario": null
                }
            ]
        },
        {
            "parameter": "SM",
            "values": [
                {
                    "value": "3,30E-04",
                    "module": "A1-A3",
                    "scenario": null
                },
                {
                    "value": "0,00E+00",
                    "module": "A4",
                    "scenario": null
                },
                {
                    "value": "0,00E+00",
                    "module": "A5",
                    "scenario": null
                },
                {
                    "value": "0,00E+00",
                    "module": "C1",
                    "scenario": null
                },
                {
                    "value": "0,00E+00",
                    "module": "C2",
                    "scenario": null
                },
                {
                    "value": "0,00E+00",
                    "module": "C3",
                    "scenario": null
                },
                {
                    "value": "0,00E+00",
                    "module": "C4",
                    "scenario": null
                },
                {
                    "value": "0,00E+00",
                    "module": "D",
                    "scenario": null
                }
            ]
        },
        {
            "parameter": "RSF",
            "values": [
                {
                    "value": "7,65E-02",
                    "module": "A1-A3",
                    "scenario": null
                },
                {
                    "value": "1,26E-04",
                    "module": "A4",
                    "scenario": null
                },
                {
                    "value": "1,74E-05",
                    "module": "A5",
                    "scenario": null
                },
                {
                    "value": "0,00E+00",
                    "module": "C1",
                    "scenario": null
                },
                {
                    "value": "0,00E+00",
                    "module": "C2",
                    "scenario": null
                },
                {
                    "value": "7,59E-05",
                    "module": "C3",
                    "scenario": null
                },
                {
                    "value": "1,14E-04",
                    "module": "C4",
                    "scenario": null
                },
                {
                    "value": "-1,22E-03",
                    "module": "D",
                    "scenario": null
                }
            ]
        },
        {
            "parameter": "NRSF",
            "values": [
                {
                    "value": "3,06E-02",
                    "module": "A1-A3",
                    "scenario": null
                },
                {
                    "value": "4,52E-04",
                    "module": "A4",
                    "scenario": null
                },
                {
                    "value": "1,56E-04",
                    "module": "A5",
                    "scenario": null
                },
                {
                    "value": "0,00E+00",
                    "module": "C1",
                    "scenario": null
                },
                {
                    "value": "0,00E+00",
                    "module": "C2",
                    "scenario": null
                },
                {
                    "value": "0,00E+00",
                    "module": "C3",
                    "scenario": null
                },
                {
                    "value": "1,83E-03",
                    "module": "C4",
                    "scenario": null
                },
                {
                    "value": "-4,14E-01",
                    "module": "D",
                    "scenario": null
                }
            ]
        },
        {
            "parameter": "FW",
            "values": [
                {
                    "value": "9,58E-02",
                    "module": "A1-A3",
                    "scenario": null
                },
                {
                    "value": "2,64E-05",
                    "module": "A4",
                    "scenario": null
                },
                {
                    "value": "1,60E-05",
                    "module": "A5",
                    "scenario": null
                },
                {
                    "value": "0,00E+00",
                    "module": "C1",
                    "scenario": null
                },
                {
                    "value": "0,00E+00",
                    "module": "C2",
                    "scenario": null
                },
                {
                    "value": "2,59E-04",
                    "module": "C3",
                    "scenario": null
                },
                {
                    "value": "1,40E-04",
                    "module": "C4",
                    "scenario": null
                },
                {
                    "value": "-8,41E-03",
                    "module": "D",
                    "scenario": null
                }
            ]
        }
    ],
    "end_of_life_waste": [
        {
            "parameter": "HWD",
            "values": [
                {
                    "value": "1,07E-02",
                    "module": "A1-A3",
                    "scenario": null
                },
                {
                    "value": "1,27E-05",
                    "module": "A4",
                    "scenario": null
                },
                {
                    "value": "1,94E-04",
                    "module": "A5",
                    "scenario": null
                },
                {
                    "value": "0,00E+00",
                    "module": "C1",
                    "scenario": null
                },
                {
                    "value": "0,00E+00",
                    "module": "C2",
                    "scenario": null
                },
                {
                    "value": "0,00E+00",
                    "module": "C3",
                    "scenario": null
                },
                {
                    "value": "1,39E-02",
                    "module": "C4",
                    "scenario": null
                },
                {
                    "value": "-5,31E-05",
                    "module": "D",
                    "scenario": null
                }
            ]
        },
        {
            "parameter": "NHWD",
            "values": [
                {
                    "value": "1,70E-01",
                    "module": "A1-A3",
                    "scenario": null
                },
                {
                    "value": "1,20E-02",
                    "module": "A4",
                    "scenario": null
                },
                {
                    "value": "7,06E-02",
                    "module": "A5",
                    "scenario": null
                },
                {
                    "value": "0,00E+00",
                    "module": "C1",
                    "scenario": null
                },
                {
                    "value": "0,00E+00",
                    "module": "C2",
                    "scenario": null
                },
                {
                    "value": "0,00E+00",
                    "module": "C3",
                    "scenario": null
                },
                {
                    "value": "4,73E-01",
                    "module": "C4",
                    "scenario": null
                },
                {
                    "value": "-2,67E-02",
                    "module": "D",
                    "scenario": null
                }
            ]
        },
        {
            "parameter": "RWD",
            "values": [
                {
                    "value": "5,70E-05",
                    "module": "A1-A3",
                    "scenario": null
                },
                {
                    "value": "1,68E-06",
                    "module": "A4",
                    "scenario": null
                },
                {
                    "value": "5,80E-09",
                    "module": "A5",
                    "scenario": null
                },
                {
                    "value": "0,00E+00",
                    "module": "C1",
                    "scenario": null
                },
                {
                    "value": "0,00E+00",
                    "module": "C2",
                    "scenario": null
                },
                {
                    "value": "0,00E+00",
                    "module": "C3",
                    "scenario": null
                },
                {
                    "value": "7,52E-07",
                    "module": "C4",
                    "scenario": null
                },
                {
                    "value": "-5,92E-06",
                    "module": "D",
                    "scenario": null
                }
            ]
        }
    ],
    "end_of_life_flow": [
        {
            "parameter": "CRU",
            "values": [
                {
                    "value": "0,00E+00",
                    "module": "A1-A3",
                    "scenario": null
                },
                {
                    "value": "0,00E+00",
                    "module": "A4",
                    "scenario": null
                },
                {
                    "value": "0,00E+00",
                    "module": "A5",
                    "scenario": null
                },
                {
                    "value": "0,00E+00",
                    "module": "C1",
                    "scenario": null
                },
                {
                    "value": "0,00E+00",
                    "module": "C2",
                    "scenario": null
                },
                {
                    "value": "0,00E+00",
                    "module": "C3",
                    "scenario": null
                },
                {
                    "value": "0,00E+00",
                    "module": "C4",
                    "scenario": null
                },
                {
                    "value": "0,00E+00",
                    "module": "D",
                    "scenario": null
                }
            ]
        },
        {
            "parameter": "MFR",
            "values": [
                {
                    "value": "8,26E-02",
                    "module": "A1-A3",
                    "scenario": null
                },
                {
                    "value": "0,00E+00",
                    "module": "A4",
                    "scenario": null
                },
                {
                    "value": "1,06E-02",
                    "module": "A5",
                    "scenario": null
                },
                {
                    "value": "0,00E+00",
                    "module": "C1",
                    "scenario": null
                },
                {
                    "value": "0,00E+00",
                    "module": "C2",
                    "scenario": null
                },
                {
                    "value": "0,00E+00",
                    "module": "C3",
                    "scenario": null
                },
                {
                    "value": "4,17E-05",
                    "module": "C4",
                    "scenario": null
                },
                {
                    "value": "0,00E+00",
                    "module": "D",
                    "scenario": null
                }
            ]
        },
        {
            "parameter": "MER",
            "values": [
                {
                    "value": "3,10E-02",
                    "module": "A1-A3",
                    "scenario": null
                },
                {
                    "value": "0,00E+00",
                    "module": "A4",
                    "scenario": null
                },
                {
                    "value": "5,00E-02",
                    "module": "A5",
                    "scenario": null
                },
                {
                    "value": "0,00E+00",
                    "module": "C1",
                    "scenario": null
                },
                {
                    "value": "0,00E+00",
                    "module": "C2",
                    "scenario": null
                },
                {
                    "value": "4,65E-01",
                    "module": "C3",
                    "scenario": null
                },
                {
                    "value": "1,02E-06",
                    "module": "C4",
                    "scenario": null
                },
                {
                    "value": "0,00E+00",
                    "module": "D",
                    "scenario": null
                }
            ]
        },
        {
            "parameter": "EEE",
            "values": [
                {
                    "value": "2,63E-02",
                    "module": "A1-A3",
                    "scenario": null
                },
                {
                    "value": "0,00E+00",
                    "module": "A4",
                    "scenario": null
                },
                {
                    "value": "3,47E-02",
                    "module": "A5",
                    "scenario": null
                },
                {
                    "value": "0,00E+00",
                    "module": "C1",
                    "scenario": null
                },
                {
                    "value": "0,00E+00",
                    "module": "C2",
                    "scenario": null
                },
                {
                    "value": "9,01E-01",
                    "module": "C3",
                    "scenario": null
                },
                {
                    "value": "6,61E-05",
                    "module": "C4",
                    "scenario": null
                },
                {
                    "value": "0,00E+00",
                    "module": "D",
                    "scenario": null
                }
            ]
        },
        {
            "parameter": "EET",
            "values": [
                {
                    "value": "3,97E-01",
                    "module": "A1-A3",
                    "scenario": null
                },
                {
                    "value": "0,00E+00",
                    "module": "A4",
                    "scenario": null
                },
                {
                    "value": "5,25E-01",
                    "module": "A5",
                    "scenario": null
                },
                {
                    "value": "0,00E+00",
                    "module": "C1",
                    "scenario": null
                },
                {
                    "value": "0,00E+00",
                    "module": "C2",
                    "scenario": null
                },
                {
                    "value": "1,36E+01",
                    "module": "C3",
                    "scenario": null
                },
                {
                    "value": "1,00E-03",
                    "module": "C4",
                    "scenario": null
                },
                {
                    "value": "0,00E+00",
                    "module": "D",
                    "scenario": null
                }
            ]
        }
    ]
}