{
    "product_name": "DBB Air insulated switchgear Type: AH12 - Comprising of Outgoing & Incoming feeders, Buscoupler & Bus sectionalizer with Transfer",
    "epd_id": "NEPD-8816-8478",
    "declared_unit": {
        "unit": "stk",
        "amount": 1.0
    },
    "compliance": [
        "EN 15804+A2",
        "ISO 14025",
        "ISO 21930"
    ],
    "producer_name": "Al-Ahleia Switchgear Co., k.s.c.c",
    "environmental_impact": [
        {
            "parameter": "GWP-total",
            "values": [
                {
                    "value": "7,07E+04",
                    "module": "A1-A3",
                    "scenario": null
                },
                {
                    "value": "5,65E+02",
                    "module": "A4",
                    "scenario": null
                },
                {
                    "value": "4,50E+02",
                    "module": "A5",
                    "scenario": null
                },
                {
                    "value": "0,00E+00",
                    "module": "B1",
                    "scenario": null
                },
                {
                    "value": "3,07E+05",
                    "module": "B6",
                    "scenario": null
                },
                {
                    "value": "0,00E+00",
                    "module": "C1",
                    "scenario": null
                },
                {
                    "value": "5,65E+02",
                    "module": "C2",
                    "scenario": null
                },
                {
                    "value": "1,47E+03",
                    "module": "C3",
                    "scenario": null
                },
                {
                    "value": "1,23E+02",
                    "module": "C4",
                    "scenario": null
                },
                {
                    "value": "-5,40E+03",
                    "module": "D",
                    "scenario": null
                }
            ]
        },
        {
            "parameter": "GWP-fossil",
            "values": [
                {
                    "value": "7,01E+04",
                    "module": "A1-A3",
                    "scenario": null
                },
                {
                    "value": "5,65E+02",
                    "module": "A4",
                    "scenario": null
                },
                {
                    "value": "8,12E+00",
                    "module": "A5",
                    "scenario": null
                },
                {
                    "value": "0,00E+00",
                    "module": "B1",
                    "scenario": null
                },
                {
                    "value": "3,07E+05",
                    "module": "B6",
                    "scenario": null
                },
                {
                    "value": "0,00E+00",
                    "module": "C1",
                    "scenario": null
                },
                {
                    "value": "5,65E+02",
                    "module": "C2",
                    "scenario": null
                },
                {
                    "value": "1,46E+03",
                    "module": "C3",
                    "scenario": null
                },
                {
                    "value": "1,23E+02",
                    "module": "C4",
                    "scenario": null
                },
                {
                    "value": "-5,38E+03",
                    "module": "D",
                    "scenario": null
                }
            ]
        },
        {
            "parameter": "GWP-biogenic",
            "values": [
                {
                    "value": "5,67E+02",
                    "module": "A1-A3",
                    "scenario": null
                },
                {
                    "value": "2,20E-01",
                    "module": "A4",
                    "scenario": null
                },
                {
                    "value": "4,42E+02",
                    "module": "A5",
                    "scenario": null
                },
                {
                    "value": "0,00E+00",
                    "module": "B1",
                    "scenario": null
                },
                {
                    "value": "2,68E+01",
                    "module": "B6",
                    "scenario": null
                },
                {
                    "value": "0,00E+00",
                    "module": "C1",
                    "scenario": null
                },
                {
                    "value": "2,20E-01",
                    "module": "C2",
                    "scenario": null
                },
                {
                    "value": "7,31E+00",
                    "module": "C3",
                    "scenario": null
                },
                {
                    "value": "2,14E-02",
                    "module": "C4",
                    "scenario": null
                },
                {
                    "value": "-1,02E+01",
                    "module": "D",
                    "scenario": null
                }
            ]
        },
        {
            "parameter": "GWP-luluc",
            "values": [
                {
                    "value": "6,22E+01",
                    "module": "A1-A3",
                    "scenario": null
                },
                {
                    "value": "2,07E-01",
                    "module": "A4",
                    "scenario": null
                },
                {
                    "value": "2,03E-03",
                    "module": "A5",
                    "scenario": null
                },
                {
                    "value": "0,00E+00",
                    "module": "B1",
                    "scenario": null
                },
                {
                    "value": "1,03E+01",
                    "module": "B6",
                    "scenario": null
                },
                {
                    "value": "0,00E+00",
                    "module": "C1",
                    "scenario": null
                },
                {
                    "value": "2,07E-01",
                    "module": "C2",
                    "scenario": null
                },
                {
                    "value": "1,24E-01",
                    "module": "C3",
                    "scenario": null
                },
                {
                    "value": "2,27E-02",
                    "module": "C4",
                    "scenario": null
                },
                {
                    "value": "-5,61E+00",
                    "module": "D",
                    "scenario": null
                }
            ]
        },
        {
            "parameter": "ODP",
            "values": [
                {
                    "value": "6,58E-03",
                    "module": "A1-A3",
                    "scenario": null
                },
                {
                    "value": "1,23E-04",
                    "module": "A4",
                    "scenario": null
                },
                {
                    "value": "1,27E-06",
                    "module": "A5",
                    "scenario": null
                },
                {
                    "value": "0,00E+00",
                    "module": "B1",
                    "scenario": null
                },
                {
                    "value": "4,97E-02",
                    "module": "B6",
                    "scenario": null
                },
                {
                    "value": "0,00E+00",
                    "module": "C1",
                    "scenario": null
                },
                {
                    "value": "1,23E-04",
                    "module": "C2",
                    "scenario": null
                },
                {
                    "value": "5,18E-05",
                    "module": "C3",
                    "scenario": null
                },
                {
                    "value": "1,28E-05",
                    "module": "C4",
                    "scenario": null
                },
                {
                    "value": "-4,52E+00",
                    "module": "D",
                    "scenario": null
                }
            ]
        },
        {
            "parameter": "AP",
            "values": [
                {
                    "value": "2,32E+03",
                    "module": "A1-A3",
                    "scenario": null
                },
                {
                    "value": "1,69E+00",
                    "module": "A4",
                    "scenario": null
                },
                {
                    "value": "6,35E-02",
                    "module": "A5",
                    "scenario": null
                },
                {
                    "value": "0,00E+00",
                    "module": "B1",
                    "scenario": null
                },
                {
                    "value": "2,26E+03",
                    "module": "B6",
                    "scenario": null
                },
                {
                    "value": "0,00E+00",
                    "module": "C1",
                    "scenario": null
                },
                {
                    "value": "1,69E+00",
                    "module": "C2",
                    "scenario": null
                },
                {
                    "value": "9,29E-01",
                    "module": "C3",
                    "scenario": null
                },
                {
                    "value": "4,21E-01",
                    "module": "C4",
                    "scenario": null
                },
                {
                    "value": "-3,09E+02",
                    "module": "D",
                    "scenario": null
                }
            ]
        },
        {
            "parameter": "POCP",
            "values": [
                {
                    "value": "5,05E+02",
                    "module": "A1-A3",
                    "scenario": null
                },
                {
                    "value": "1,39E+00",
                    "module": "A4",
                    "scenario": null
                },
                {
                    "value": "7,50E-02",
                    "module": "A5",
                    "scenario": null
                },
                {
                    "value": "0,00E+00",
                    "module": "B1",
                    "scenario": null
                },
                {
                    "value": "1,02E+03",
                    "module": "B6",
                    "scenario": null
                },
                {
                    "value": "0,00E+00",
                    "module": "C1",
                    "scenario": null
                },
                {
                    "value": "1,39E+00",
                    "module": "C2",
                    "scenario": null
                },
                {
                    "value": "7,22E-01",
                    "module": "C3",
                    "scenario": null
                },
                {
                    "value": "4,66E-01",
                    "module": "C4",
                    "scenario": null
                },
                {
                    "value": "-6,88E+01",
                    "module": "D",
                    "scenario": null
                }
            ]
        },
        {
            "parameter": "ADPE",
            "values": [
                {
                    "value": "2,10E+01",
                    "module": "A1-A3",
                    "scenario": null
                },
                {
                    "value": "1,52E-02",
                    "module": "A4",
                    "scenario": null
                },
                {
                    "value": "1,29E-04",
                    "module": "A5",
                    "scenario": null
                },
                {
                    "value": "0,00E+00",
                    "module": "B1",
                    "scenario": null
                },
                {
                    "value": "3,10E-01",
                    "module": "B6",
                    "scenario": null
                },
                {
                    "value": "0,00E+00",
                    "module": "C1",
                    "scenario": null
                },
                {
                    "value": "1,52E-02",
                    "module": "C2",
                    "scenario": null
                },
                {
                    "value": "1,81E-03",
                    "module": "C3",
                    "scenario": null
                },
                {
                    "value": "3,76E-04",
                    "module": "C4",
                    "scenario": null
                },
                {
                    "value": "-1,71E+00",
                    "module": "D",
                    "scenario": null
                }
            ]
        },
        {
            "parameter": "ADPF",
            "values": [
                {
                    "value": "8,52E+05",
                    "module": "A1-A3",
                    "scenario": null
                },
                {
                    "value": "8,35E+03",
                    "module": "A4",
                    "scenario": null
                },
                {
                    "value": "9,34E+01",
                    "module": "A5",
                    "scenario": null
                },
                {
                    "value": "0,00E+00",
                    "module": "B1",
                    "scenario": null
                },
                {
                    "value": "4,15E+06",
                    "module": "B6",
                    "scenario": null
                },
                {
                    "value": "0,00E+00",
                    "module": "C1",
                    "scenario": null
                },
                {
                    "value": "8,35E+03",
                    "module": "C2",
                    "scenario": null
                },
                {
                    "value": "2,70E+03",
                    "module": "C3",
                    "scenario": null
                },
                {
                    "value": "1,09E+03",
                    "module": "C4",
                    "scenario": null
                },
                {
                    "value": "-4,66E+04",
                    "module": "D",
                    "scenario": null
                }
            ]
        },
        {
            "parameter": "WDP",
            "values": [
                {
                    "value": "3,72E+05",
                    "module": "A1-A3",
                    "scenario": null
                },
                {
                    "value": "2,72E+03",
                    "module": "A4",
                    "scenario": null
                },
                {
                    "value": "1,46E+02",
                    "module": "A5",
                    "scenario": null
                },
                {
                    "value": "0,00E+00",
                    "module": "B1",
                    "scenario": null
                },
                {
                    "value": "1,51E+06",
                    "module": "B6",
                    "scenario": null
                },
                {
                    "value": "0,00E+00",
                    "module": "C1",
                    "scenario": null
                },
                {
                    "value": "2,72E+03",
                    "module": "C2",
                    "scenario": null
                },
                {
                    "value": "1,14E+04",
                    "module": "C3",
                    "scenario": null
                },
                {
                    "value": "2,52E+04",
                    "module": "C4",
                    "scenario": null
                },
                {
                    "value": "2,69E+05",
                    "module": "D",
                    "scenario": null
                }
            ]
        },
        {
            "parameter": "EP-freshwater",
            "values": [
                {
                    "value": "2,10E+01",
                    "module": "A1-A3",
                    "scenario": null
                },
                {
                    "value": "5,30E-03",
                    "module": "A4",
                    "scenario": null
                },
                {
                    "value": "9,46E-05",
                    "module": "A5",
                    "scenario": null
                },
                {
                    "value": "0,00E+00",
                    "module": "B1",
                    "scenario": null
                },
                {
                    "value": "4,69E-01",
                    "module": "B6",
                    "scenario": null
                },
                {
                    "value": "0,00E+00",
                    "module": "C1",
                    "scenario": null
                },
                {
                    "value": "5,30E-03",
                    "module": "C2",
                    "scenario": null
                },
                {
                    "value": "3,58E-03",
                    "module": "C3",
                    "scenario": null
                },
                {
                    "value": "1,20E-03",
                    "module": "C4",
                    "scenario": null
                },
                {
                    "value": "-2,19E+00",
                    "module": "D",
                    "scenario": null
                }
            ]
        },
        {
            "parameter": "EP-marine",
            "values": [
                {
                    "value": "1,27E+02",
                    "module": "A1-A3",
                    "scenario": null
                },
                {
                    "value": "3,33E-01",
                    "module": "A4",
                    "scenario": null
                },
                {
                    "value": "2,74E-02",
                    "module": "A5",
                    "scenario": null
                },
                {
                    "value": "0,00E+00",
                    "module": "B1",
                    "scenario": null
                },
                {
                    "value": "3,23E+02",
                    "module": "B6",
                    "scenario": null
                },
                {
                    "value": "0,00E+00",
                    "module": "C1",
                    "scenario": null
                },
                {
                    "value": "3,33E-01",
                    "module": "C2",
                    "scenario": null
                },
                {
                    "value": "2,32E-01",
                    "module": "C3",
                    "scenario": null
                },
                {
                    "value": "2,00E-01",
                    "module": "C4",
                    "scenario": null
                },
                {
                    "value": "-1,58E+01",
                    "module": "D",
                    "scenario": null
                }
            ]
        },
        {
            "parameter": "EP-terrestrial",
            "values": [
                {
                    "value": "1,90E+03",
                    "module": "A1-A3",
                    "scenario": null
                },
                {
                    "value": "3,72E+00",
                    "module": "A4",
                    "scenario": null
                },
                {
                    "value": "2,91E-01",
                    "module": "A5",
                    "scenario": null
                },
                {
                    "value": "0,00E+00",
                    "module": "B1",
                    "scenario": null
                },
                {
                    "value": "3,54E+03",
                    "module": "B6",
                    "scenario": null
                },
                {
                    "value": "0,00E+00",
                    "module": "C1",
                    "scenario": null
                },
                {
                    "value": "3,72E+00",
                    "module": "C2",
                    "scenario": null
                },
                {
                    "value": "2,50E+00",
                    "module": "C3",
                    "scenario": null
                },
                {
                    "value": "1,67E+00",
                    "module": "C4",
                    "scenario": null
                },
                {
                    "value": "-2,25E+02",
                    "module": "D",
                    "scenario": null
                }
            ]
        }
    ],
    "additional_environmental_impact": [
        {
            "parameter": "PM",
            "values": [
                {
                    "value": "7,18E-03",
                    "module": "A1-A3",
                    "scenario": null
                },
                {
                    "value": "3,65E-05",
                    "module": "A4",
                    "scenario": null
                },
                {
                    "value": "7,78E-07",
                    "module": "A5",
                    "scenario": null
                },
                {
                    "value": "0,00E+00",
                    "module": "B1",
                    "scenario": null
                },
                {
                    "value": "1,64E-02",
                    "module": "B6",
                    "scenario": null
                },
                {
                    "value": "0,00E+00",
                    "module": "C1",
                    "scenario": null
                },
                {
                    "value": "3,65E-05",
                    "module": "C2",
                    "scenario": null
                },
                {
                    "value": "1,24E-05",
                    "module": "C3",
                    "scenario": null
                },
                {
                    "value": "7,74E-06",
                    "module": "C4",
                    "scenario": null
                },
                {
                    "value": "-9,11E-04",
                    "module": "D",
                    "scenario": null
                }
            ]
        },
        {
            "parameter": "ETP-fw",
            "values": [
                {
                    "value": "1,65E+07",
                    "module": "A1-A3",
                    "scenario": null
                },
                {
                    "value": "6,77E+03",
                    "module": "A4",
                    "scenario": null
                },
                {
                    "value": "1,06E+02",
                    "module": "A5",
                    "scenario": null
                },
                {
                    "value": "0,00E+00",
                    "module": "B1",
                    "scenario": null
                },
                {
                    "value": "1,53E+06",
                    "module": "B6",
                    "scenario": null
                },
                {
                    "value": "0,00E+00",
                    "module": "C1",
                    "scenario": null
                },
                {
                    "value": "6,77E+03",
                    "module": "C2",
                    "scenario": null
                },
                {
                    "value": "9,64E+03",
                    "module": "C3",
                    "scenario": null
                },
                {
                    "value": "1,48E+06",
                    "module": "C4",
                    "scenario": null
                },
                {
                    "value": "-2,88E+06",
                    "module": "D",
                    "scenario": null
                }
            ]
        },
        {
            "parameter": "HTP-c",
            "values": [
                {
                    "value": "5,26E-04",
                    "module": "A1-A3",
                    "scenario": null
                },
                {
                    "value": "0,00E+00",
                    "module": "A4",
                    "scenario": null
                },
                {
                    "value": "1,17E-08",
                    "module": "A5",
                    "scenario": null
                },
                {
                    "value": "0,00E+00",
                    "module": "B1",
                    "scenario": null
                },
                {
                    "value": "9,16E-05",
                    "module": "B6",
                    "scenario": null
                },
                {
                    "value": "0,00E+00",
                    "module": "C1",
                    "scenario": null
                },
                {
                    "value": "0,00E+00",
                    "module": "C2",
                    "scenario": null
                },
                {
                    "value": "1,26E-07",
                    "module": "C3",
                    "scenario": null
                },
                {
                    "value": "1,23E-07",
                    "module": "C4",
                    "scenario": null
                },
                {
                    "value": "-5,51E-05",
                    "module": "D",
                    "scenario": null
                }
            ]
        },
        {
            "parameter": "HTP-nc",
            "values": [
                {
                    "value": "3,26E-02",
                    "module": "A1-A3",
                    "scenario": null
                },
                {
                    "value": "6,64E-06",
                    "module": "A4",
                    "scenario": null
                },
                {
                    "value": "5,62E-07",
                    "module": "A5",
                    "scenario": null
                },
                {
                    "value": "0,00E+00",
                    "module": "B1",
                    "scenario": null
                },
                {
                    "value": "8,99E-04",
                    "module": "B6",
                    "scenario": null
                },
                {
                    "value": "0,00E+00",
                    "module": "C1",
                    "scenario": null
                },
                {
                    "value": "6,64E-06",
                    "module": "C2",
                    "scenario": null
                },
                {
                    "value": "5,46E-06",
                    "module": "C3",
                    "scenario": null
                },
                {
                    "value": "2,55E-06",
                    "module": "C4",
                    "scenario": null
                },
                {
                    "value": "-2,87E-03",
                    "module": "D",
                    "scenario": null
                }
            ]
        },
        {
            "parameter": "SQP",
            "values": [
                {
                    "value": "3,86E+05",
                    "module": "A1-A3",
                    "scenario": null
                },
                {
                    "value": "5,72E+03",
                    "module": "A4",
                    "scenario": null
                },
                {
                    "value": "5,36E+01",
                    "module": "A5",
                    "scenario": null
                },
                {
                    "value": "0,00E+00",
                    "module": "B1",
                    "scenario": null
                },
                {
                    "value": "4,10E+05",
                    "module": "B6",
                    "scenario": null
                },
                {
                    "value": "0,00E+00",
                    "module": "C1",
                    "scenario": null
                },
                {
                    "value": "5,72E+03",
                    "module": "C2",
                    "scenario": null
                },
                {
                    "value": "1,20E+03",
                    "module": "C3",
                    "scenario": null
                },
                {
                    "value": "2,25E+03",
                    "module": "C4",
                    "scenario": null
                },
                {
                    "value": "-4,22E+04",
                    "module": "D",
                    "scenario": null
                }
            ]
        },
        {
            "parameter": "IRP",
            "values": [
                {
                    "value": "2,24E+03",
                    "module": "A1-A3",
                    "scenario": null
                },
                {
                    "value": "3,47E+01",
                    "module": "A4",
                    "scenario": null
                },
                {
                    "value": "3,39E-01",
                    "module": "A5",
                    "scenario": null
                },
                {
                    "value": "0,00E+00",
                    "module": "B1",
                    "scenario": null
                },
                {
                    "value": "1,24E+04",
                    "module": "B6",
                    "scenario": null
                },
                {
                    "value": "0,00E+00",
                    "module": "C1",
                    "scenario": null
                },
                {
                    "value": "3,47E+01",
                    "module": "C2",
                    "scenario": null
                },
                {
                    "value": "1,24E+01",
                    "module": "C3",
                    "scenario": null
                },
                {
                    "value": "6,83E+00",
                    "module": "C4",
                    "scenario": null
                },
                {
                    "value": "-1,23E+01",
                    "module": "D",
                    "scenario": null
                }
            ]
        }
    ],
    "resource_use": [
        {
            "parameter": "PERE",
            "values": [
                {
                    "value": "6,76E+04",
                    "module": "A1-A3",
                    "scenario": null
                },
                {
                    "value": "9,45E+01",
                    "module": "A4",
                    "scenario": null
                },
                {
                    "value": "1,92E+00",
                    "module": "A5",
                    "scenario": null
                },
                {
                    "value": "0,00E+00",
                    "module": "B1",
                    "scenario": null
                },
                {
                    "value": "1,30E+04",
                    "module": "B6",
                    "scenario": null
                },
                {
                    "value": "0,00E+00",
                    "module": "C1",
                    "scenario": null
                },
                {
                    "value": "9,45E+01",
                    "module": "C2",
                    "scenario": null
                },
                {
                    "value": "5,26E+02",
                    "module": "C3",
                    "scenario": null
                },
                {
                    "value": "1,37E+02",
                    "module": "C4",
                    "scenario": null
                },
                {
                    "value": "-1,41E+04",
                    "module": "D",
                    "scenario": null
                }
            ]
        },
        {
            "parameter": "PERM",
            "values": [
                {
                    "value": "4,10E+03",
                    "module": "A1-A3",
                    "scenario": null
                },
                {
                    "value": "0,00E+00",
                    "module": "A4",
                    "scenario": null
                },
                {
                    "value": "-4,05E+03",
                    "module": "A5",
                    "scenario": null
                },
                {
                    "value": "0,00E+00",
                    "module": "B1",
                    "scenario": null
                },
                {
                    "value": "0,00E+00",
                    "module": "B6",
                    "scenario": null
                },
                {
                    "value": "0,00E+00",
                    "module": "C1",
                    "scenario": null
                },
                {
                    "value": "0,00E+00",
                    "module": "C2",
                    "scenario": null
                },
                {
                    "value": "-4,57E+01",
                    "module": "C3",
                    "scenario": null
                },
                {
                    "value": "0,00E+00",
                    "module": "C4",
                    "scenario": null
                },
                {
                    "value": "0,00E+00",
                    "module": "D",
                    "scenario": null
                }
            ]
        },
        {
            "parameter": "PERT",
            "values": [
                {
                    "value": "7,17E+04",
                    "module": "A1-A3",
                    "scenario": null
                },
                {
                    "value": "9,45E+01",
                    "module": "A4",
                    "scenario": null
                },
                {
                    "value": "-4,05E+03",
                    "module": "A5",
                    "scenario": null
                },
                {
                    "value": "0,00E+00",
                    "module": "B1",
                    "scenario": null
                },
                {
                    "value": "1,30E+04",
                    "module": "B6",
                    "scenario": null
                },
                {
                    "value": "0,00E+00",
                    "module": "C1",
                    "scenario": null
                },
                {
                    "value": "9,45E+01",
                    "module": "C2",
                    "scenario": null
                },
                {
                    "value": "4,80E+02",
                    "module": "C3",
                    "scenario": null
                },
                {
                    "value": "1,37E+02",
                    "module": "C4",
                    "scenario": null
                },
                {
                    "value": "-1,41E+04",
                    "module": "D",
                    "scenario": null
                }
            ]
        },
        {
            "parameter": "PENRE",
            "values": [
                {
                    "value": "8,46E+05",
                    "module": "A1-A3",
                    "scenario": null
                },
                {
                    "value": "8,35E+03",
                    "module": "A4",
                    "scenario": null
                },
                {
                    "value": "9,34E+01",
                    "module": "A5",
                    "scenario": null
                },
                {
                    "value": "0,00E+00",
                    "module": "B1",
                    "scenario": null
                },
                {
                    "value": "4,15E+06",
                    "module": "B6",
                    "scenario": null
                },
                {
                    "value": "0,00E+00",
                    "module": "C1",
                    "scenario": null
                },
                {
                    "value": "8,35E+03",
                    "module": "C2",
                    "scenario": null
                },
                {
                    "value": "2,70E+03",
                    "module": "C3",
                    "scenario": null
                },
                {
                    "value": "1,09E+03",
                    "module": "C4",
                    "scenario": null
                },
                {
                    "value": "-4,66E+04",
                    "module": "D",
                    "scenario": null
                }
            ]
        },
        {
            "parameter": "PENRM",
            "values": [
                {
                    "value": "1,36E+04",
                    "module": "A1-A3",
                    "scenario": null
                },
                {
                    "value": "0,00E+00",
                    "module": "A4",
                    "scenario": null
                },
                {
                    "value": "-1,42E+02",
                    "module": "A5",
                    "scenario": null
                },
                {
                    "value": "0,00E+00",
                    "module": "B1",
                    "scenario": null
                },
                {
                    "value": "0,00E+00",
                    "module": "B6",
                    "scenario": null
                },
                {
                    "value": "0,00E+00",
                    "module": "C1",
                    "scenario": null
                },
                {
                    "value": "0,00E+00",
                    "module": "C2",
                    "scenario": null
                },
                {
                    "value": "-1,34E+04",
                    "module": "C3",
                    "scenario": null
                },
                {
                    "value": "0,00E+00",
                    "module": "C4",
                    "scenario": null
                },
                {
                    "value": "0,00E+00",
                    "module": "D",
                    "scenario": null
                }
            ]
        },
        {
            "parameter": "PENRT",
            "values": [
                {
                    "value": "8,60E+05",
                    "module": "A1-A3",
                    "scenario": null
                },
                {
                    "value": "8,35E+03",
                    "module": "A4",
                    "scenario": null
                },
                {
                    "value": "-4,89E+01",
                    "module": "A5",
                    "scenario": null
                },
                {
                    "value": "0,00E+00",
                    "module": "B1",
                    "scenario": null
                },
                {
                    "value": "4,15E+06",
                    "module": "B6",
                    "scenario": null
                },
                {
                    "value": "0,00E+00",
                    "module": "C1",
                    "scenario": null
                },
                {
                    "value": "8,35E+03",
                    "module": "C2",
                    "scenario": null
                },
                {
                    "value": "-1,07E+04",
                    "module": "C3",
                    "scenario": null
                },
                {
                    "value": "1,09E+03",
                    "module": "C4",
                    "scenario": null
                },
                {
                    "value": "-4,66E+04",
                    "module": "D",
                    "scenario": null
                }
            ]
        },
        {
            "parameter": "SM",
            "values": [
                {
                    "value": "3,60E+03",
                    "module": "A1-A3",
                    "scenario": null
                },
                {
                    "value": "0,00E+00",
                    "module": "A4",
                    "scenario": null
                },
                {
                    "value": "0,00E+00",
                    "module": "A5",
                    "scenario": null
                },
                {
                    "value": "0,00E+00",
                    "module": "B1",
                    "scenario": null
                },
                {
                    "value": "0,00E+00",
                    "module": "B6",
                    "scenario": null
                },
                {
                    "value": "0,00E+00",
                    "module": "C1",
                    "scenario": null
                },
                {
                    "value": "0,00E+00",
                    "module": "C2",
                    "scenario": null
                },
                {
                    "value": "0,00E+00",
                    "module": "C3",
                    "scenario": null
                },
                {
                    "value": "5,08E-02",
                    "module": "C4",
                    "scenario": null
                },
                {
                    "value": "5,06E+02",
                    "module": "D",
                    "scenario": null
                }
            ]
        },
        {
            "parameter": "RSF",
            "values": [
                {
                    "value": "5,46E+02",
                    "module": "A1-A3",
                    "scenario": null
                },
                {
                    "value": "1,85E+00",
                    "module": "A4",
                    "scenario": null
                },
                {
                    "value": "5,60E-02",
                    "module": "A5",
                    "scenario": null
                },
                {
                    "value": "0,00E+00",
                    "module": "B1",
                    "scenario": null
                },
                {
                    "value": "2,39E+02",
                    "module": "B6",
                    "scenario": null
                },
                {
                    "value": "0,00E+00",
                    "module": "C1",
                    "scenario": null
                },
                {
                    "value": "1,85E+00",
                    "module": "C2",
                    "scenario": null
                },
                {
                    "value": "1,11E+01",
                    "module": "C3",
                    "scenario": null
                },
                {
                    "value": "2,88E+00",
                    "module": "C4",
                    "scenario": null
                },
                {
                    "value": "1,77E+02",
                    "module": "D",
                    "scenario": null
                }
            ]
        },
        {
            "parameter": "NRSF",
            "values": [
                {
                    "value": "1,27E+04",
                    "module": "A1-A3",
                    "scenario": null
                },
                {
                    "value": "1,57E+01",
                    "module": "A4",
                    "scenario": null
                },
                {
                    "value": "6,32E-01",
                    "module": "A5",
                    "scenario": null
                },
                {
                    "value": "0,00E+00",
                    "module": "B1",
                    "scenario": null
                },
                {
                    "value": "1,22E+03",
                    "module": "B6",
                    "scenario": null
                },
                {
                    "value": "0,00E+00",
                    "module": "C1",
                    "scenario": null
                },
                {
                    "value": "1,57E+01",
                    "module": "C2",
                    "scenario": null
                },
                {
                    "value": "0,00E+00",
                    "module": "C3",
                    "scenario": null
                },
                {
                    "value": "3,71E+00",
                    "module": "C4",
                    "scenario": null
                },
                {
                    "value": "3,55E+03",
                    "module": "D",
                    "scenario": null
                }
            ]
        },
        {
            "parameter": "FW",
            "values": [
                {
                    "value": "6,64E+02",
                    "module": "A1-A3",
                    "scenario": null
                },
                {
                    "value": "9,34E-01",
                    "module": "A4",
                    "scenario": null
                },
                {
                    "value": "6,77E-02",
                    "module": "A5",
                    "scenario": null
                },
                {
                    "value": "0,00E+00",
                    "module": "B1",
                    "scenario": null
                },
                {
                    "value": "7,09E+02",
                    "module": "B6",
                    "scenario": null
                },
                {
                    "value": "0,00E+00",
                    "module": "C1",
                    "scenario": null
                },
                {
                    "value": "9,34E-01",
                    "module": "C2",
                    "scenario": null
                },
                {
                    "value": "2,35E+00",
                    "module": "C3",
                    "scenario": null
                },
                {
                    "value": "1,45E+00",
                    "module": "C4",
                    "scenario": null
                },
                {
                    "value": "-5,66E+01",
                    "module": "D",
                    "scenario": null
                }
            ]
        }
    ],
    "end_of_life_waste": [
        {
            "parameter": "HWD",
            "values": [
                {
                    "value": "5,09E+02",
                    "module": "A1-A3",
                    "scenario": null
                },
                {
                    "value": "7,54E-01",
                    "module": "A4",
                    "scenario": null
                },
                {
                    "value": "0,00E+00",
                    "module": "A5",
                    "scenario": null
                },
                {
                    "value": "0,00E+00",
                    "module": "B1",
                    "scenario": null
                },
                {
                    "value": "3,71E+02",
                    "module": "B6",
                    "scenario": null
                },
                {
                    "value": "0,00E+00",
                    "module": "C1",
                    "scenario": null
                },
                {
                    "value": "7,54E-01",
                    "module": "C2",
                    "scenario": null
                },
                {
                    "value": "0,00E+00",
                    "module": "C3",
                    "scenario": null
                },
                {
                    "value": "9,47E+01",
                    "module": "C4",
                    "scenario": null
                },
                {
                    "value": "-3,83E+01",
                    "module": "D",
                    "scenario": null
                }
            ]
        },
        {
            "parameter": "NHWD",
            "values": [
                {
                    "value": "1,60E+04",
                    "module": "A1-A3",
                    "scenario": null
                },
                {
                    "value": "4,01E+02",
                    "module": "A4",
                    "scenario": null
                },
                {
                    "value": "2,95E+02",
                    "module": "A5",
                    "scenario": null
                },
                {
                    "value": "0,00E+00",
                    "module": "B1",
                    "scenario": null
                },
                {
                    "value": "4,36E+03",
                    "module": "B6",
                    "scenario": null
                },
                {
                    "value": "0,00E+00",
                    "module": "C1",
                    "scenario": null
                },
                {
                    "value": "4,01E+02",
                    "module": "C2",
                    "scenario": null
                },
                {
                    "value": "1,05E+01",
                    "module": "C3",
                    "scenario": null
                },
                {
                    "value": "3,01E+03",
                    "module": "C4",
                    "scenario": null
                },
                {
                    "value": "-2,32E+03",
                    "module": "D",
                    "scenario": null
                }
            ]
        },
        {
            "parameter": "RWD",
            "values": [
                {
                    "value": "2,72E+00",
                    "module": "A1-A3",
                    "scenario": null
                },
                {
                    "value": "5,48E-02",
                    "module": "A4",
                    "scenario": null
                },
                {
                    "value": "0,00E+00",
                    "module": "A5",
                    "scenario": null
                },
                {
                    "value": "0,00E+00",
                    "module": "B1",
                    "scenario": null
                },
                {
                    "value": "2,02E+01",
                    "module": "B6",
                    "scenario": null
                },
                {
                    "value": "0,00E+00",
                    "module": "C1",
                    "scenario": null
                },
                {
                    "value": "5,48E-02",
                    "module": "C2",
                    "scenario": null
                },
                {
                    "value": "0,00E+00",
                    "module": "C3",
                    "scenario": null
                },
                {
                    "value": "6,24E-03",
                    "module": "C4",
                    "scenario": null
                },
                {
                    "value": "-1,24E-02",
                    "module": "D",
                    "scenario": null
                }
            ]
        }
    ],
    "end_of_life_flow": [
        {
            "parameter": "CRU",
            "values": [
                {
                    "value": "0,00E+00",
                    "module": "A1-A3",
                    "scenario": null
                },
                {
                    "value": "0,00E+00",
                    "module": "A4",
                    "scenario": null
                },
                {
                    "value": "0,00E+00",
                    "module": "A5",
                    "scenario": null
                },
                {
                    "value": "0,00E+00",
                    "module": "B1",
                    "scenario": null
                },
                {
                    "value": "0,00E+00",
                    "module": "B6",
                    "scenario": null
                },
                {
                    "value": "0,00E+00",
                    "module": "C1",
                    "scenario": null
                },
                {
                    "value": "0,00E+00",
                    "module": "C2",
                    "scenario": null
                },
                {
                    "value": "0,00E+00",
                    "module": "C3",
                    "scenario": null
                },
                {
                    "value": "0,00E+00",
                    "module": "C4",
                    "scenario": null
                },
                {
                    "value": "0,00E+00",
                    "module": "D",
                    "scenario": null
                }
            ]
        },
        {
            "parameter": "MFR",
            "values": [
                {
                    "value": "2,32E+03",
                    "module": "A1-A3",
                    "scenario": null
                },
                {
                    "value": "0,00E+00",
                    "module": "A4",
                    "scenario": null
                },
                {
                    "value": "1,72E+00",
                    "module": "A5",
                    "scenario": null
                },
                {
                    "value": "0,00E+00",
                    "module": "B1",
                    "scenario": null
                },
                {
                    "value": "0,00E+00",
                    "module": "B6",
                    "scenario": null
                },
                {
                    "value": "0,00E+00",
                    "module": "C1",
                    "scenario": null
                },
                {
                    "value": "0,00E+00",
                    "module": "C2",
                    "scenario": null
                },
                {
                    "value": "7,24E+03",
                    "module": "C3",
                    "scenario": null
                },
                {
                    "value": "4,09E-02",
                    "module": "C4",
                    "scenario": null
                },
                {
                    "value": "-1,99E+01",
                    "module": "D",
                    "scenario": null
                }
            ]
        },
        {
            "parameter": "MER",
            "values": [
                {
                    "value": "2,48E+02",
                    "module": "A1-A3",
                    "scenario": null
                },
                {
                    "value": "0,00E+00",
                    "module": "A4",
                    "scenario": null
                },
                {
                    "value": "2,92E+02",
                    "module": "A5",
                    "scenario": null
                },
                {
                    "value": "0,00E+00",
                    "module": "B1",
                    "scenario": null
                },
                {
                    "value": "0,00E+00",
                    "module": "B6",
                    "scenario": null
                },
                {
                    "value": "0,00E+00",
                    "module": "C1",
                    "scenario": null
                },
                {
                    "value": "0,00E+00",
                    "module": "C2",
                    "scenario": null
                },
                {
                    "value": "6,36E+02",
                    "module": "C3",
                    "scenario": null
                },
                {
                    "value": "1,00E-03",
                    "module": "C4",
                    "scenario": null
                },
                {
                    "value": "-2,61E+00",
                    "module": "D",
                    "scenario": null
                }
            ]
        },
        {
            "parameter": "EEE",
            "values": [
                {
                    "value": "1,44E+02",
                    "module": "A1-A3",
                    "scenario": null
                },
                {
                    "value": "0,00E+00",
                    "module": "A4",
                    "scenario": null
                },
                {
                    "value": "2,03E+02",
                    "module": "A5",
                    "scenario": null
                },
                {
                    "value": "0,00E+00",
                    "module": "B1",
                    "scenario": null
                },
                {
                    "value": "0,00E+00",
                    "module": "B6",
                    "scenario": null
                },
                {
                    "value": "0,00E+00",
                    "module": "C1",
                    "scenario": null
                },
                {
                    "value": "0,00E+00",
                    "module": "C2",
                    "scenario": null
                },
                {
                    "value": "7,01E+02",
                    "module": "C3",
                    "scenario": null
                },
                {
                    "value": "6,49E-02",
                    "module": "C4",
                    "scenario": null
                },
                {
                    "value": "-6,42E+00",
                    "module": "D",
                    "scenario": null
                }
            ]
        },
        {
            "parameter": "EET",
            "values": [
                {
                    "value": "2,17E+03",
                    "module": "A1-A3",
                    "scenario": null
                },
                {
                    "value": "0,00E+00",
                    "module": "A4",
                    "scenario": null
                },
                {
                    "value": "3,07E+03",
                    "module": "A5",
                    "scenario": null
                },
                {
                    "value": "0,00E+00",
                    "module": "B1",
                    "scenario": null
                },
                {
                    "value": "0,00E+00",
                    "module": "B6",
                    "scenario": null
                },
                {
                    "value": "0,00E+00",
                    "module": "C1",
                    "scenario": null
                },
                {
                    "value": "0,00E+00",
                    "module": "C2",
                    "scenario": null
                },
                {
                    "value": "1,06E+04",
                    "module": "C3",
                    "scenario": null
                },
                {
                    "value": "9,82E-01",
                    "module": "C4",
                    "scenario": null
                },
                {
                    "value": "-9,72E+01",
                    "module": "D",
                    "scenario": null
                }
            ]
        }
    ]
}