{"product_name":"Tufted modular carpet tiles with CQuest Bio backing, aqueous dyed surface and a max. total pile material of 1500 g/m\u00b2 PA 6 with 100% recycled content","epd_id":"EPD-INT-20210152-CBB2-EN","compliance":["DIN EN 15804","ISO 14025"],"producer_name":"Interface Europe Manufacturing BV","environmental_impact":[{"parameter":"GWP-total","unit":"kg CO2-eq.","values":[{"value":"5,26E+00","module":"A1-A3"},{"value":"3,19E-01","module":"A4"},{"value":"5,93E-01","module":"A5"},{"value":"0,0E+00","module":"B1"},{"value":"2,91E-01","module":"B2"},{"value":"4,45E-02","module":"C2"},{"value":"7,03E+00","module":"C3"},{"value":"7,11E+00","module":"C3"},{"value":"1,26E+00","module":"C4"},{"value":"-1,95E-02","module":"D"},{"value":"0,0E+00","module":"D"},{"value":"-3,27E-01","module":"D"},{"value":"-2,41E-01","module":"D"}]},{"parameter":"ODP","unit":"kg CFC11-eq.","values":[{"value":"2,74E-08","module":"A1-A3"},{"value":"5,56E-17","module":"A4"},{"value":"8,22E-10","module":"A5"},{"value":"0,0E+00","module":"B1"},{"value":"1,21E-08","module":"B2"},{"value":"7,76E-18","module":"C2"},{"value":"2,55E-15","module":"C3"},{"value":"3,50E-15","module":"C3"},{"value":"1,23E-15","module":"C4"},{"value":"-2,99E-16","module":"D"},{"value":"0,0E+00","module":"D"},{"value":"-4,93E-15","module":"D"},{"value":"-1,46E-15","module":"D"}]},{"parameter":"AP","unit":"kg SO2-eq.","values":[{"value":"2,33E-02","module":"A1-A3"},{"value":"1,32E-03","module":"A4"},{"value":"8,93E-04","module":"A5"},{"value":"0,0E+00","module":"B1"},{"value":"1,14E-03","module":"B2"},{"value":"1,84E-04","module":"C2"},{"value":"4,99E-03","module":"C3"},{"value":"5,24E-03","module":"C3"},{"value":"9,44E-04","module":"C4"},{"value":"-2,27E-05","module":"D"},{"value":"0,0E+00","module":"D"},{"value":"-3,75E-04","module":"D"},{"value":"-8,63E-04","module":"D"}]},{"parameter":"EP","unit":"kg PO4^3-eq.","values":[{"value":"5,95E-03","module":"A1-A3"},{"value":"3,36E-04","module":"A4"},{"value":"2,27E-04","module":"A5"},{"value":"0,0E+00","module":"B1"},{"value":"3,16E-04","module":"B2"},{"value":"4,68E-05","module":"C2"},{"value":"1,26E-03","module":"C3"},{"value":"1,31E-03","module":"C3"},{"value":"1,03E-03","module":"C4"},{"value":"-3,11E-06","module":"D"},{"value":"0,0E+00","module":"D"},{"value":"-5,17E-05","module":"D"},{"value":"-1,13E-04","module":"D"}]},{"parameter":"POCP","unit":"kg Ethen-eq.","values":[{"value":"1,42E-03","module":"A1-A3"},{"value":"-5,64E-04","module":"A4"},{"value":"3,37E-05","module":"A5"},{"value":"6,29E-05","module":"B1"},{"value":"1,47E-04","module":"B2"},{"value":"-7,88E-05","module":"C2"},{"value":"3,03E-04","module":"C3"},{"value":"2,28E-04","module":"C3"},{"value":"8,50E-05","module":"C4"},{"value":"-2,08E-06","module":"D"},{"value":"0,0E+00","module":"D"},{"value":"-3,46E-05","module":"D"},{"value":"-8,03E-05","module":"D"}]},{"parameter":"ADPE","unit":"kg Sb-eq.","values":[{"value":"9,95E-06","module":"A1-A3"},{"value":"2,83E-08","module":"A4"},{"value":"3,06E-07","module":"A5"},{"value":"0,0E+00","module":"B1"},{"value":"4,43E-06","module":"B2"},{"value":"3,94E-09","module":"C2"},{"value":"2,31E-07","module":"C3"},{"value":"2,45E-07","module":"C3"},{"value":"6,98E-08","module":"C4"},{"value":"-3,67E-09","module":"D"},{"value":"0,0E+00","module":"D"},{"value":"-6,07E-08","module":"D"},{"value":"-1,90E-07","module":"D"}]},{"parameter":"ADPF","unit":"MJ","values":[{"value":"1,07E+02","module":"A1-A3"},{"value":"4,34E+00","module":"A4"},{"value":"3,48E+00","module":"A5"},{"value":"0,0E+00","module":"B1"},{"value":"6,77E+00","module":"B2"},{"value":"6,06E-01","module":"C2"},{"value":"3,85E+00","module":"C3"},{"value":"4,79E+00","module":"C3"},{"value":"5,44E+00","module":"C4"},{"value":"-2,81E-01","module":"D"},{"value":"0,0E+00","module":"D"},{"value":"-4,71E+00","module":"D"},{"value":"-2,16E+01","module":"D"}]}],"additional_environmental_impact":[],"resource_use":[{"parameter":"PERE","unit":"MJ","values":[{"value":"8,49E+01","module":"A1-A3"},{"value":"2,43E-01","module":"A4"},{"value":"3,37E+00","module":"A5"},{"value":"0,0E+00","module":"B1"},{"value":"1,24E+00","module":"B2"},{"value":"3,38E-02","module":"C2"},{"value":"1,47E+01","module":"C3"},{"value":"1,49E+01","module":"C3"},{"value":"4,06E-01","module":"C4"},{"value":"-7,71E-02","module":"D"},{"value":"0,0E+00","module":"D"},{"value":"-1,27E+00","module":"D"},{"value":"-3,42E-01","module":"D"}]},{"parameter":"PERM","unit":"MJ","values":[{"value":"1,44E+01","module":"A1-A3"},{"value":"0,0E+00","module":"A4"},{"value":"-3,63E-01","module":"A5"},{"value":"0,0E+00","module":"B1"},{"value":"0,0E+00","module":"B2"},{"value":"0,0E+00","module":"C2"},{"value":"-1,41E+01","module":"C3"},{"value":"-1,41E+01","module":"C3"},{"value":"0,0E+00","module":"C4"},{"value":"0,0E+00","module":"D"},{"value":"0,0E+00","module":"D"},{"value":"0,0E+00","module":"D"},{"value":"0,0E+00","module":"D"}]},{"parameter":"PERT","unit":"MJ","values":[{"value":"9,94E+01","module":"A1-A3"},{"value":"2,43E-01","module":"A4"},{"value":"3,01E+00","module":"A5"},{"value":"0,0E+00","module":"B1"},{"value":"1,24E+00","module":"B2"},{"value":"3,38E-02","module":"C2"},{"value":"5,99E-01","module":"C3"},{"value":"8,75E-01","module":"C3"},{"value":"4,06E-01","module":"C4"},{"value":"-7,71E-02","module":"D"},{"value":"0,0E+00","module":"D"},{"value":"-1,27E+00","module":"D"},{"value":"-3,42E-01","module":"D"}]},{"parameter":"PENRE","unit":"MJ","values":[{"value":"1,05E+02","module":"A1-A3"},{"value":"4,35E+00","module":"A4"},{"value":"3,95E+00","module":"A5"},{"value":"0,0E+00","module":"B1"},{"value":"7,86E+00","module":"B2"},{"value":"6,07E-01","module":"C2"},{"value":"1,29E+01","module":"C3"},{"value":"1,40E+01","module":"C3"},{"value":"5,60E+00","module":"C4"},{"value":"-3,43E-01","module":"D"},{"value":"0,0E+00","module":"D"},{"value":"-5,74E+00","module":"D"},{"value":"-2,18E+01","module":"D"}]},{"parameter":"PENRM","unit":"MJ","values":[{"value":"8,95E+00","module":"A1-A3"},{"value":"0,0E+00","module":"A4"},{"value":"-2,75E-01","module":"A5"},{"value":"0,0E+00","module":"B1"},{"value":"0,0E+00","module":"B2"},{"value":"0,0E+00","module":"C2"},{"value":"-8,68E+00","module":"C3"},{"value":"-8,68E+00","module":"C3"},{"value":"0,0E+00","module":"C4"},{"value":"0,0E+00","module":"D"},{"value":"0,0E+00","module":"D"},{"value":"0,0E+00","module":"D"},{"value":"0,0E+00","module":"D"}]},{"parameter":"PENRT","unit":"MJ","values":[{"value":"1,14E+02","module":"A1-A3"},{"value":"4,35E+00","module":"A4"},{"value":"3,67E+00","module":"A5"},{"value":"0,0E+00","module":"B1"},{"value":"7,86E+00","module":"B2"},{"value":"6,07E-01","module":"C2"},{"value":"4,21E+00","module":"C3"},{"value":"5,34E+00","module":"C3"},{"value":"5,60E+00","module":"C4"},{"value":"-3,43E-01","module":"D"},{"value":"0,0E+00","module":"D"},{"value":"-5,74E+00","module":"D"},{"value":"-2,18E+01","module":"D"}]},{"parameter":"SM","unit":"kg","values":[{"value":"4,28E+00","module":"A1-A3"},{"value":"0,0E+00","module":"A4"},{"value":"1,28E-01","module":"A5"},{"value":"0,0E+00","module":"B1"},{"value":"0,0E+00","module":"B2"},{"value":"0,0E+00","module":"C2"},{"value":"0,0E+00","module":"C3"},{"value":"0,0E+00","module":"C3"},{"value":"0,0E+00","module":"C4"},{"value":"0,0E+00","module":"D"},{"value":"0,0E+00","module":"D"},{"value":"0,0E+00","module":"D"},{"value":"2,60E-01","module":"D"}]},{"parameter":"RSF","unit":"MJ","values":[{"value":"0,0E+00","module":"A1-A3"},{"value":"0,0E+00","module":"A4"},{"value":"0,0E+00","module":"A5"},{"value":"0,0E+00","module":"B1"},{"value":"0,0E+00","module":"B2"},{"value":"0,0E+00","module":"C2"},{"value":"0,0E+00","module":"C3"},{"value":"0,0E+00","module":"C3"},{"value":"0,0E+00","module":"C4"},{"value":"0,0E+00","module":"D"},{"value":"0,0E+00","module":"D"},{"value":"0,0E+00","module":"D"},{"value":"0,0E+00","module":"D"}]},{"parameter":"NRSF","unit":"MJ","values":[{"value":"0,0E+00","module":"A1-A3"},{"value":"0,0E+00","module":"A4"},{"value":"0,0E+00","module":"A5"},{"value":"0,0E+00","module":"B1"},{"value":"0,0E+00","module":"B2"},{"value":"0,0E+00","module":"C2"},{"value":"0,0E+00","module":"C3"},{"value":"0,0E+00","module":"C3"},{"value":"0,0E+00","module":"C4"},{"value":"0,0E+00","module":"D"},{"value":"0,0E+00","module":"D"},{"value":"0,0E+00","module":"D"},{"value":"0,0E+00","module":"D"}]},{"parameter":"FW","unit":"m^3","values":[{"value":"4,93E-01","module":"A1-A3"},{"value":"2,78E-04","module":"A4"},{"value":"1,55E-02","module":"A5"},{"value":"0,0E+00","module":"B1"},{"value":"4,13E-03","module":"B2"},{"value":"3,87E-05","module":"C2"},{"value":"2,03E-02","module":"C3"},{"value":"2,06E-02","module":"C3"},{"value":"5,16E-05","module":"C4"},{"value":"-7,53E-05","module":"D"},{"value":"0,0E+00","module":"D"},{"value":"-1,24E-03","module":"D"},{"value":"-2,06E-03","module":"D"}]}],"end_of_life_waste":[{"parameter":"HWD","unit":"kg","values":[{"value":"4,23E-03","module":"A1-A3"},{"value":"2,19E-10","module":"A4"},{"value":"1,27E-04","module":"A5"},{"value":"0,0E+00","module":"B1"},{"value":"5,90E-10","module":"B2"},{"value":"3,06E-11","module":"C2"},{"value":"1,69E-08","module":"C3"},{"value":"1,71E-08","module":"C3"},{"value":"1,01E-09","module":"C4"},{"value":"-7,70E-11","module":"D"},{"value":"0,0E+00","module":"D"},{"value":"-1,29E-09","module":"D"},{"value":"-1,67E-09","module":"D"}]},{"parameter":"NHWD","unit":"kg","values":[{"value":"8,09E-01","module":"A1-A3"},{"value":"6,47E-04","module":"A4"},{"value":"6,87E-02","module":"A5"},{"value":"0,0E+00","module":"B1"},{"value":"5,62E-03","module":"B2"},{"value":"9,02E-05","module":"C2"},{"value":"1,48E+00","module":"C3"},{"value":"1,48E+00","module":"C3"},{"value":"5,34E+00","module":"C4"},{"value":"-1,60E-04","module":"D"},{"value":"0,0E+00","module":"D"},{"value":"-2,67E-03","module":"D"},{"value":"-1,62E-01","module":"D"}]},{"parameter":"RWD","unit":"kg","values":[{"value":"2,19E-03","module":"A1-A3"},{"value":"5,27E-06","module":"A4"},{"value":"7,03E-05","module":"A5"},{"value":"0,0E+00","module":"B1"},{"value":"3,31E-04","module":"B2"},{"value":"7,35E-07","module":"C2"},{"value":"1,42E-04","module":"C3"},{"value":"2,21E-04","module":"C3"},{"value":"6,50E-05","module":"C4"},{"value":"-2,48E-05","module":"D"},{"value":"0,0E+00","module":"D"},{"value":"-4,09E-04","module":"D"},{"value":"-8,83E-05","module":"D"}]}],"end_of_life_flow":[{"parameter":"CRU","unit":"kg","values":[{"value":"0,0E+00","module":"A1-A3"},{"value":"0,0E+00","module":"A4"},{"value":"0,0E+00","module":"A5"},{"value":"0,0E+00","module":"B1"},{"value":"0,0E+00","module":"B2"},{"value":"0,0E+00","module":"C2"},{"value":"0,0E+00","module":"C3"},{"value":"0,0E+00","module":"C3"},{"value":"0,0E+00","module":"C4"},{"value":"0,0E+00","module":"D"},{"value":"0,0E+00","module":"D"},{"value":"0,0E+00","module":"D"},{"value":"0,0E+00","module":"D"}]},{"parameter":"MFR","unit":"kg","values":[{"value":"0,0E+00","module":"A1-A3"},{"value":"0,0E+00","module":"A4"},{"value":"1,21E-01","module":"A5"},{"value":"0,0E+00","module":"B1"},{"value":"0,0E+00","module":"B2"},{"value":"0,0E+00","module":"C2"},{"value":"0,0E+00","module":"C3"},{"value":"1,70E+00","module":"C3"},{"value":"0,0E+00","module":"C4"},{"value":"0,0E+00","module":"D"},{"value":"0,0E+00","module":"D"},{"value":"0,0E+00","module":"D"},{"value":"0,0E+00","module":"D"}]},{"parameter":"MER","unit":"kg","values":[{"value":"0,0E+00","module":"A1-A3"},{"value":"0,0E+00","module":"A4"},{"value":"0,0E+00","module":"A5"},{"value":"0,0E+00","module":"B1"},{"value":"0,0E+00","module":"B2"},{"value":"0,0E+00","module":"C2"},{"value":"0,0E+00","module":"C3"},{"value":"0,0E+00","module":"C3"},{"value":"0,0E+00","module":"C4"},{"value":"0,0E+00","module":"D"},{"value":"0,0E+00","module":"D"},{"value":"0,0E+00","module":"D"},{"value":"0,0E+00","module":"D"}]},{"parameter":"EEE","unit":"MJ","values":[{"value":"0,0E+00","module":"A1-A3"},{"value":"0,0E+00","module":"A4"},{"value":"2,78E-01","module":"A5"},{"value":"0,0E+00","module":"B1"},{"value":"0,0E+00","module":"B2"},{"value":"0,0E+00","module":"C2"},{"value":"7,85E+00","module":"C3"},{"value":"0,0E+00","module":"C3"},{"value":"0,0E+00","module":"C4"},{"value":"0,0E+00","module":"D"},{"value":"0,0E+00","module":"D"},{"value":"0,0E+00","module":"D"},{"value":"0,0E+00","module":"D"}]},{"parameter":"EET","unit":"MJ","values":[{"value":"0,0E+00","module":"A1-A3"},{"value":"0,0E+00","module":"A4"},{"value":"5,17E-01","module":"A5"},{"value":"0,0E+00","module":"B1"},{"value":"0,0E+00","module":"B2"},{"value":"0,0E+00","module":"C2"},{"value":"1,47E+01","module":"C3"},{"value":"7,45E+01","module":"C3"},{"value":"0,0E+00","module":"C4"},{"value":"0,0E+00","module":"D"},{"value":"0,0E+00","module":"D"},{"value":"0,0E+00","module":"D"},{"value":"0,0E+00","module":"D"}]}]}