{"product_name":"Tufted modular carpet tiles with CQuest Bio backing and a pile material of PA 6.6 with 75% recycled content","epd_id":"EPD-INT-20200180-CCC1-EN","declared_unit":{"unit":"m2","amount":1},"compliance":["DIN EN 15804","ISO 14025"],"producer_name":"Interface Europe Manufacturing BV","environmental_impact":[{"parameter":"GWP-total","unit":"kg CO2-eq","values":[{"value":"6,51E+00","module":"A1-A3","scenario":null},{"value":"2,63E-01","module":"A4","scenario":null},{"value":"4,21E-01","module":"A5","scenario":null},{"value":"0,00E+00","module":"B1","scenario":null},{"value":"2,92E-01","module":"B2","scenario":null},{"value":"1,46E-02","module":"C2","scenario":null},{"value":"5,67E+00","module":"C3","scenario":"S2"},{"value":"5,73E+00","module":"C3","scenario":"S3"},{"value":"1,20E+00","module":"C4","scenario":null},{"value":"-2,52E-02","module":"D","scenario":"S0"},{"value":"0,00E+00","module":"D","scenario":"S1"},{"value":"-5,11E-01","module":"D","scenario":"S2"},{"value":"-2,55E-01","module":"D","scenario":"S3"}]},{"parameter":"ODP","unit":"kg CFC11-eq","values":[{"value":"2,44E-08","module":"A1-A3","scenario":null},{"value":"4,33E-17","module":"A4","scenario":null},{"value":"7,33E-10","module":"A5","scenario":null},{"value":"0,00E+00","module":"B1","scenario":null},{"value":"1,21E-08","module":"B2","scenario":null},{"value":"2,40E-18","module":"C2","scenario":null},{"value":"2,01E-15","module":"C3","scenario":"S2"},{"value":"2,74E-15","module":"C3","scenario":"S3"},{"value":"9,66E-16","module":"C4","scenario":null},{"value":"-3,56E-16","module":"D","scenario":"S0"},{"value":"0,00E+00","module":"D","scenario":"S1"},{"value":"-7,17E-15","module":"D","scenario":"S2"},{"value":"-1,32E-15","module":"D","scenario":"S3"}]},{"parameter":"AP","unit":"mol H+-eq","values":[{"value":"1,68E-02","module":"A1-A3","scenario":null},{"value":"1,11E-03","module":"A4","scenario":null},{"value":"6,44E-04","module":"A5","scenario":null},{"value":"0,00E+00","module":"B1","scenario":null},{"value":"1,16E-03","module":"B2","scenario":null},{"value":"6,17E-05","module":"C2","scenario":null},{"value":"3,47E-03","module":"C3","scenario":"S2"},{"value":"3,68E-03","module":"C3","scenario":"S3"},{"value":"8,08E-04","module":"C4","scenario":null},{"value":"-3,17E-05","module":"D","scenario":"S0"},{"value":"0,00E+00","module":"D","scenario":"S1"},{"value":"-6,42E-04","module":"D","scenario":"S2"},{"value":"-9,44E-04","module":"D","scenario":"S3"}]},{"parameter":"EP","unit":"kg PO_4^3-eq","values":[{"value":"1,08E-02","module":"A1-A3","scenario":null},{"value":"2,79E-04","module":"A4","scenario":null},{"value":"3,58E-04","module":"A5","scenario":null},{"value":"0,00E+00","module":"B1","scenario":null},{"value":"3,17E-04","module":"B2","scenario":null},{"value":"1,55E-05","module":"C2","scenario":null},{"value":"8,59E-04","module":"C3","scenario":"S2"},{"value":"9,03E-04","module":"C3","scenario":"S3"},{"value":"8,45E-04","module":"C4","scenario":null},{"value":"-3,95E-06","module":"D","scenario":"S0"},{"value":"0,00E+00","module":"D","scenario":"S1"},{"value":"-8,00E-05","module":"D","scenario":"S2"},{"value":"-1,17E-04","module":"D","scenario":"S3"}]},{"parameter":"POCP","unit":"kg NMVOC-eq","values":[{"value":"1,37E-03","module":"A1-A3","scenario":null},{"value":"-4,68E-04","module":"A4","scenario":null},{"value":"3,25E-05","module":"A5","scenario":null},{"value":"6,29E-05","module":"B1","scenario":null},{"value":"1,48E-04","module":"B2","scenario":null},{"value":"-2,60E-05","module":"C2","scenario":null},{"value":"2,12E-04","module":"C3","scenario":"S2"},{"value":"1,50E-04","module":"C3","scenario":"S3"},{"value":"9,12E-05","module":"C4","scenario":null},{"value":"-2,89E-06","module":"D","scenario":"S0"},{"value":"0,00E+00","module":"D","scenario":"S1"},{"value":"-5,86E-05","module":"D","scenario":"S2"},{"value":"-9,12E-05","module":"D","scenario":"S3"}]},{"parameter":"ADPE","unit":"kg Sb-eq","values":[{"value":"1,33E-05","module":"A1-A3","scenario":null},{"value":"2,23E-08","module":"A4","scenario":null},{"value":"4,07E-07","module":"A5","scenario":null},{"value":"0,00E+00","module":"B1","scenario":null},{"value":"4,43E-06","module":"B2","scenario":null},{"value":"1,24E-09","module":"C2","scenario":null},{"value":"1,95E-07","module":"C3","scenario":"S2"},{"value":"2,06E-07","module":"C3","scenario":"S3"},{"value":"5,77E-08","module":"C4","scenario":null},{"value":"-4,70E-09","module":"D","scenario":"S0"},{"value":"0,00E+00","module":"D","scenario":"S1"},{"value":"-9,50E-08","module":"D","scenario":"S2"},{"value":"-1,42E-07","module":"D","scenario":"S3"}]},{"parameter":"ADPF","unit":"MJ","values":[{"value":"1,23E+02","module":"A1-A3","scenario":null},{"value":"3,59E+00","module":"A4","scenario":null},{"value":"3,88E+00","module":"A5","scenario":null},{"value":"0,00E+00","module":"B1","scenario":null},{"value":"6,76E+00","module":"B2","scenario":null},{"value":"1,99E-01","module":"C2","scenario":null},{"value":"2,94E+00","module":"C3","scenario":"S2"},{"value":"3,71E+00","module":"C3","scenario":"S3"},{"value":"4,45E+00","module":"C4","scenario":null},{"value":"-3,53E-01","module":"D","scenario":"S0"},{"value":"0,00E+00","module":"D","scenario":"S1"},{"value":"-7,18E+00","module":"D","scenario":"S2"},{"value":"-2,80E+01","module":"D","scenario":"S3"}]}],"additional_environmental_impact":[],"resource_use":[{"parameter":"PERE","unit":"MJ","values":[{"value":"3,16E+01","module":"A1-A3","scenario":null},{"value":"2,02E-01","module":"A4","scenario":null},{"value":"1,72E+00","module":"A5","scenario":null},{"value":"0,00E+00","module":"B1","scenario":null},{"value":"1,20E+00","module":"B2","scenario":null},{"value":"1,12E-02","module":"C2","scenario":null},{"value":"1,38E+01","module":"C3","scenario":"S2"},{"value":"1,40E+01","module":"C3","scenario":"S3"},{"value":"3,22E-01","module":"C4","scenario":null},{"value":"-9,47E-02","module":"D","scenario":"S0"},{"value":"0,00E+00","module":"D","scenario":"S1"},{"value":"-1,91E+00","module":"D","scenario":"S2"},{"value":"-3,13E-01","module":"D","scenario":"S3"}]},{"parameter":"PERM","unit":"","values":[{"value":"1,36E+01","module":"A1-A3","scenario":null},{"value":"0,00E+00","module":"A4","scenario":null},{"value":"-3,39E-01","module":"A5","scenario":null},{"value":"0,00E+00","module":"B1","scenario":null},{"value":"0,00E+00","module":"B2","scenario":null},{"value":"0,00E+00","module":"C2","scenario":null},{"value":"-1,33E+01","module":"C3","scenario":"S2"},{"value":"-1,33E+01","module":"C3","scenario":"S3"},{"value":"0,00E+00","module":"C4","scenario":null},{"value":"0,00E+00","module":"D","scenario":"S0"},{"value":"0,00E+00","module":"D","scenario":"S1"},{"value":"0,00E+00","module":"D","scenario":"S2"},{"value":"0,00E+00","module":"D","scenario":"S3"}]},{"parameter":"PERT","unit":"MJ","values":[{"value":"4,52E+01","module":"A1-A3","scenario":null},{"value":"2,02E-01","module":"A4","scenario":null},{"value":"1,38E+00","module":"A5","scenario":null},{"value":"0,00E+00","module":"B1","scenario":null},{"value":"1,20E+00","module":"B2","scenario":null},{"value":"1,12E-02","module":"C2","scenario":null},{"value":"4,78E-01","module":"C3","scenario":"S2"},{"value":"6,99E-01","module":"C3","scenario":"S3"},{"value":"3,22E-01","module":"C4","scenario":null},{"value":"-9,47E-02","module":"D","scenario":"S0"},{"value":"0,00E+00","module":"D","scenario":"S1"},{"value":"-1,91E+00","module":"D","scenario":"S2"},{"value":"-3,13E-01","module":"D","scenario":"S3"}]},{"parameter":"PENRE","unit":"MJ","values":[{"value":"1,18E+02","module":"A1-A3","scenario":null},{"value":"3,60E+00","module":"A4","scenario":null},{"value":"4,55E+00","module":"A5","scenario":null},{"value":"0,00E+00","module":"B1","scenario":null},{"value":"7,86E+00","module":"B2","scenario":null},{"value":"2,00E-01","module":"C2","scenario":null},{"value":"2,04E+01","module":"C3","scenario":"S2"},{"value":"2,13E+01","module":"C3","scenario":"S3"},{"value":"4,59E+00","module":"C4","scenario":null},{"value":"-4,35E-01","module":"D","scenario":"S0"},{"value":"0,00E+00","module":"D","scenario":"S1"},{"value":"-8,82E+00","module":"D","scenario":"S2"},{"value":"-2,82E+01","module":"D","scenario":"S3"}]},{"parameter":"PENRM","unit":"MJ","values":[{"value":"1,74E+01","module":"A1-A3","scenario":null},{"value":"0,00E+00","module":"A4","scenario":null},{"value":"-2,69E-01","module":"A5","scenario":null},{"value":"0,00E+00","module":"B1","scenario":null},{"value":"0,00E+00","module":"B2","scenario":null},{"value":"0,00E+00","module":"C2","scenario":null},{"value":"-1,71E+01","module":"C3","scenario":"S2"},{"value":"-1,71E+01","module":"C3","scenario":"S3"},{"value":"0,00E+00","module":"C4","scenario":null},{"value":"0,00E+00","module":"D","scenario":"S0"},{"value":"0,00E+00","module":"D","scenario":"S1"},{"value":"0,00E+00","module":"D","scenario":"S2"},{"value":"0,00E+00","module":"D","scenario":"S3"}]},{"parameter":"PENRT","unit":"MJ","values":[{"value":"1,35E+02","module":"A1-A3","scenario":null},{"value":"3,60E+00","module":"A4","scenario":null},{"value":"4,28E+00","module":"A5","scenario":null},{"value":"0,00E+00","module":"B1","scenario":null},{"value":"7,86E+00","module":"B2","scenario":null},{"value":"2,00E-01","module":"C2","scenario":null},{"value":"3,24E+00","module":"C3","scenario":"S2"},{"value":"4,18E+00","module":"C3","scenario":"S3"},{"value":"4,59E+00","module":"C4","scenario":null},{"value":"-4,35E-01","module":"D","scenario":"S0"},{"value":"0,00E+00","module":"D","scenario":"S1"},{"value":"-8,82E+00","module":"D","scenario":"S2"},{"value":"-2,82E+01","module":"D","scenario":"S3"}]},{"parameter":"SM","unit":"kg","values":[{"value":"3,37E+00","module":"A1-A3","scenario":null},{"value":"0,00E+00","module":"A4","scenario":null},{"value":"1,01E-01","module":"A5","scenario":null},{"value":"0,00E+00","module":"B1","scenario":null},{"value":"0,00E+00","module":"B2","scenario":null},{"value":"0,00E+00","module":"C2","scenario":null},{"value":"0,00E+00","module":"C3","scenario":"S2"},{"value":"0,00E+00","module":"C3","scenario":"S3"},{"value":"0,00E+00","module":"C4","scenario":null},{"value":"0,00E+00","module":"D","scenario":"S0"},{"value":"0,00E+00","module":"D","scenario":"S1"},{"value":"0,00E+00","module":"D","scenario":"S2"},{"value":"1,90E-01","module":"D","scenario":"S3"}]},{"parameter":"RSF","unit":"MJ","values":[{"value":"0,00E+00","module":"A1-A3","scenario":null},{"value":"0,00E+00","module":"A4","scenario":null},{"value":"0,00E+00","module":"A5","scenario":null},{"value":"0,00E+00","module":"B1","scenario":null},{"value":"0,00E+00","module":"B2","scenario":null},{"value":"0,00E+00","module":"C2","scenario":null},{"value":"0,00E+00","module":"C3","scenario":"S2"},{"value":"0,00E+00","module":"C3","scenario":"S3"},{"value":"0,00E+00","module":"C4","scenario":null},{"value":"0,00E+00","module":"D","scenario":"S0"},{"value":"0,00E+00","module":"D","scenario":"S1"},{"value":"0,00E+00","module":"D","scenario":"S2"},{"value":"0,00E+00","module":"D","scenario":"S3"}]},{"parameter":"NRSF","unit":"MJ","values":[{"value":"0,00E+00","module":"A1-A3","scenario":null},{"value":"0,00E+00","module":"A4","scenario":null},{"value":"0,00E+00","module":"A5","scenario":null},{"value":"0,00E+00","module":"B1","scenario":null},{"value":"0,00E+00","module":"B2","scenario":null},{"value":"0,00E+00","module":"C2","scenario":null},{"value":"0,00E+00","module":"C3","scenario":"S2"},{"value":"0,00E+00","module":"C3","scenario":"S3"},{"value":"0,00E+00","module":"C4","scenario":null},{"value":"0,00E+00","module":"D","scenario":"S0"},{"value":"0,00E+00","module":"D","scenario":"S1"},{"value":"0,00E+00","module":"D","scenario":"S2"},{"value":"0,00E+00","module":"D","scenario":"S3"}]},{"parameter":"FW","unit":"m3","values":[{"value":"3,38E-01","module":"A1-A3","scenario":null},{"value":"2,34E-04","module":"A4","scenario":null},{"value":"1,07E-02","module":"A5","scenario":null},{"value":"0,00E+00","module":"B1","scenario":null},{"value":"4,27E-03","module":"B2","scenario":null},{"value":"1,30E-05","module":"C2","scenario":null},{"value":"1,62E-02","module":"C3","scenario":"S2"},{"value":"1,65E-02","module":"C3","scenario":"S3"},{"value":"5,63E-05","module":"C4","scenario":null},{"value":"-1,10E-04","module":"D","scenario":"S0"},{"value":"0,00E+00","module":"D","scenario":"S1"},{"value":"-2,21E-03","module":"D","scenario":"S2"},{"value":"-2,50E-03","module":"D","scenario":"S3"}]}],"end_of_life_waste":[{"parameter":"HWD","unit":"kg","values":[{"value":"4,16E-07","module":"A1-A3","scenario":null},{"value":"1,68E-07","module":"A4","scenario":null},{"value":"1,84E-08","module":"A5","scenario":null},{"value":"0,00E+00","module":"B1","scenario":null},{"value":"9,63E-10","module":"B2","scenario":null},{"value":"9,30E-09","module":"C2","scenario":null},{"value":"1,65E-08","module":"C3","scenario":"S2"},{"value":"3,99E-08","module":"C3","scenario":"S3"},{"value":"1,67E-08","module":"C4","scenario":null},{"value":"-1,73E-10","module":"D","scenario":"S0"},{"value":"0,00E+00","module":"D","scenario":"S1"},{"value":"-3,52E-09","module":"D","scenario":"S2"},{"value":"-6,47E-09","module":"D","scenario":"S3"}]},{"parameter":"NHWD","unit":"kg","values":[{"value":"3,46E-01","module":"A1-A3","scenario":null},{"value":"5,51E-04","module":"A4","scenario":null},{"value":"4,94E-02","module":"A5","scenario":null},{"value":"0,00E+00","module":"B1","scenario":null},{"value":"5,63E-03","module":"B2","scenario":null},{"value":"3,06E-05","module":"C2","scenario":null},{"value":"1,30E+00","module":"C3","scenario":"S2"},{"value":"1,30E+00","module":"C3","scenario":"S3"},{"value":"4,40E+00","module":"C4","scenario":null},{"value":"-2,01E-04","module":"D","scenario":"S0"},{"value":"0,00E+00","module":"D","scenario":"S1"},{"value":"-4,06E-03","module":"D","scenario":"S2"},{"value":"-1,16E-01","module":"D","scenario":"S3"}]},{"parameter":"RWD","unit":"kg","values":[{"value":"4,84E-03","module":"A1-A3","scenario":null},{"value":"4,45E-06","module":"A4","scenario":null},{"value":"1,49E-04","module":"A5","scenario":null},{"value":"0,00E+00","module":"B1","scenario":null},{"value":"3,38E-04","module":"B2","scenario":null},{"value":"2,47E-07","module":"C2","scenario":null},{"value":"1,18E-04","module":"C3","scenario":"S2"},{"value":"1,84E-04","module":"C3","scenario":"S3"},{"value":"5,53E-05","module":"C4","scenario":null},{"value":"-3,23E-05","module":"D","scenario":"S0"},{"value":"0,00E+00","module":"D","scenario":"S1"},{"value":"-6,52E-04","module":"D","scenario":"S2"},{"value":"-8,06E-05","module":"D","scenario":"S3"}]}],"end_of_life_flow":[{"parameter":"CRU","unit":"kg","values":[{"value":"0,00E+00","module":"A1-A3","scenario":null},{"value":"0,00E+00","module":"A4","scenario":null},{"value":"0,00E+00","module":"A5","scenario":null},{"value":"0,00E+00","module":"B1","scenario":null},{"value":"0,00E+00","module":"B2","scenario":null},{"value":"0,00E+00","module":"C2","scenario":null},{"value":"0,00E+00","module":"C3","scenario":"S2"},{"value":"0,00E+00","module":"C3","scenario":"S3"},{"value":"0,00E+00","module":"C4","scenario":null},{"value":"0,00E+00","module":"D","scenario":"S0"},{"value":"0,00E+00","module":"D","scenario":"S1"},{"value":"0,00E+00","module":"D","scenario":"S2"},{"value":"0,00E+00","module":"D","scenario":"S3"}]},{"parameter":"MFR","unit":"kg","values":[{"value":"0,00E+00","module":"A1-A3","scenario":null},{"value":"0,00E+00","module":"A4","scenario":null},{"value":"1,21E-01","module":"A5","scenario":null},{"value":"0,00E+00","module":"B1","scenario":null},{"value":"0,00E+00","module":"B2","scenario":null},{"value":"0,00E+00","module":"C2","scenario":null},{"value":"0,00E+00","module":"C3","scenario":"S2"},{"value":"1,44E+00","module":"C3","scenario":"S3"},{"value":"0,00E+00","module":"C4","scenario":null},{"value":"0,00E+00","module":"D","scenario":"S0"},{"value":"0,00E+00","module":"D","scenario":"S1"},{"value":"0,00E+00","module":"D","scenario":"S2"},{"value":"0,00E+00","module":"D","scenario":"S3"}]},{"parameter":"MER","unit":"kg","values":[{"value":"0,00E+00","module":"A1-A3","scenario":null},{"value":"0,00E+00","module":"A4","scenario":null},{"value":"0,00E+00","module":"A5","scenario":null},{"value":"0,00E+00","module":"B1","scenario":null},{"value":"0,00E+00","module":"B2","scenario":null},{"value":"0,00E+00","module":"C2","scenario":null},{"value":"0,00E+00","module":"C3","scenario":"S2"},{"value":"0,00E+00","module":"C3","scenario":"S3"},{"value":"0,00E+00","module":"C4","scenario":null},{"value":"0,00E+00","module":"D","scenario":"S0"},{"value":"0,00E+00","module":"D","scenario":"S1"},{"value":"0,00E+00","module":"D","scenario":"S2"},{"value":"0,00E+00","module":"D","scenario":"S3"}]},{"parameter":"EEE","unit":"MJ","values":[{"value":"0,00E+00","module":"A1-A3","scenario":null},{"value":"0,00E+00","module":"A4","scenario":null},{"value":"2,07E-01","module":"A5","scenario":null},{"value":"0,00E+00","module":"B1","scenario":null},{"value":"0,00E+00","module":"B2","scenario":null},{"value":"0,00E+00","module":"C2","scenario":null},{"value":"5,49E+00","module":"C3","scenario":"S2"},{"value":"0,00E+00","module":"C3","scenario":"S3"},{"value":"0,00E+00","module":"C4","scenario":null},{"value":"0,00E+00","module":"D","scenario":"S0"},{"value":"0,00E+00","module":"D","scenario":"S1"},{"value":"0,00E+00","module":"D","scenario":"S2"},{"value":"0,00E+00","module":"D","scenario":"S3"}]},{"parameter":"EET","unit":"MJ","values":[{"value":"0,00E+00","module":"A1-A3","scenario":null},{"value":"0,00E+00","module":"A4","scenario":null},{"value":"3,88E-01","module":"A5","scenario":null},{"value":"0,00E+00","module":"B1","scenario":null},{"value":"0,00E+00","module":"B2","scenario":null},{"value":"0,00E+00","module":"C2","scenario":null},{"value":"1,04E+01","module":"C3","scenario":"S2"},{"value":"6,33E+01","module":"C3","scenario":"S3"},{"value":"0,00E+00","module":"C4","scenario":null},{"value":"0,00E+00","module":"D","scenario":"S0"},{"value":"0,00E+00","module":"D","scenario":"S1"},{"value":"0,00E+00","module":"D","scenario":"S2"},{"value":"0,00E+00","module":"D","scenario":"S3"}]}]}