{"product_name":"Component EPD Surnadal: PVC insulated and PVC sheathed house wiring cable for open, fixed installation indoors and outdoors PR 2x2,5/2,5","epd_id":"NEPD-8140-7806","declared_unit":{"unit":"ton","amount":1},"compliance":["EN 15804+A2","ISO 14025","ISO 21930"],"producer_name":"Pipelife Norge AS","environmental_impact":[{"parameter":"GWP-total","unit":"kg CO2-eq","values":[{"value":"3,94E+00","module":"A1-A3","scenario":null},{"value":"1,63E-02","module":"A4","scenario":null},{"value":"0,00E+00","module":"C1","scenario":null},{"value":"0,00E+00","module":"C2","scenario":null},{"value":"0,00E+00","module":"C3","scenario":null},{"value":"0,00E+00","module":"C4","scenario":null},{"value":"0,00E+00","module":"D","scenario":null}]},{"parameter":"GWP-fossil","unit":"kg CO2-eq","values":[{"value":"3,91E+00","module":"A1-A3","scenario":null},{"value":"1,63E-02","module":"A4","scenario":null},{"value":"0,00E+00","module":"C1","scenario":null},{"value":"0,00E+00","module":"C2","scenario":null},{"value":"0,00E+00","module":"C3","scenario":null},{"value":"0,00E+00","module":"C4","scenario":null},{"value":"0,00E+00","module":"D","scenario":null}]},{"parameter":"GWP-biogenic","unit":"kg CO2-eq","values":[{"value":"1,88E-02","module":"A1-A3","scenario":null},{"value":"6,76E-06","module":"A4","scenario":null},{"value":"0,00E+00","module":"C1","scenario":null},{"value":"0,00E+00","module":"C2","scenario":null},{"value":"0,00E+00","module":"C3","scenario":null},{"value":"0,00E+00","module":"C4","scenario":null},{"value":"0,00E+00","module":"D","scenario":null}]},{"parameter":"GWP-luluc","unit":"kg CO2-eq","values":[{"value":"1,21E-02","module":"A1-A3","scenario":null},{"value":"5,81E-06","module":"A4","scenario":null},{"value":"0,00E+00","module":"C1","scenario":null},{"value":"0,00E+00","module":"C2","scenario":null},{"value":"0,00E+00","module":"C3","scenario":null},{"value":"0,00E+00","module":"C4","scenario":null},{"value":"0,00E+00","module":"D","scenario":null}]},{"parameter":"ODP","unit":"kg CFC11-eq","values":[{"value":"3,71E-08","module":"A1-A3","scenario":null},{"value":"3,70E-09","module":"A4","scenario":null},{"value":"0,00E+00","module":"C1","scenario":null},{"value":"0,00E+00","module":"C2","scenario":null},{"value":"0,00E+00","module":"C3","scenario":null},{"value":"0,00E+00","module":"C4","scenario":null},{"value":"0,00E+00","module":"D","scenario":null}]},{"parameter":"AP","unit":"mol H+-eq","values":[{"value":"4,06E-02","module":"A1-A3","scenario":null},{"value":"4,69E-05","module":"A4","scenario":null},{"value":"0,00E+00","module":"C1","scenario":null},{"value":"0,00E+00","module":"C2","scenario":null},{"value":"0,00E+00","module":"C3","scenario":null},{"value":"0,00E+00","module":"C4","scenario":null},{"value":"0,00E+00","module":"D","scenario":null}]},{"parameter":"POCP","unit":"kg NMVOC-eq","values":[{"value":"1,14E-02","module":"A1-A3","scenario":null},{"value":"3,98E-05","module":"A4","scenario":null},{"value":"0,00E+00","module":"C1","scenario":null},{"value":"0,00E+00","module":"C2","scenario":null},{"value":"0,00E+00","module":"C3","scenario":null},{"value":"0,00E+00","module":"C4","scenario":null},{"value":"0,00E+00","module":"D","scenario":null}]},{"parameter":"ADPE","unit":"kg Sb-eq","values":[{"value":"1,58E-03","module":"A1-A3","scenario":null},{"value":"4,51E-07","module":"A4","scenario":null},{"value":"0,00E+00","module":"C1","scenario":null},{"value":"0,00E+00","module":"C2","scenario":null},{"value":"0,00E+00","module":"C3","scenario":null},{"value":"0,00E+00","module":"C4","scenario":null},{"value":"0,00E+00","module":"D","scenario":null}]},{"parameter":"ADPF","unit":"MJ","values":[{"value":"6,29E+01","module":"A1-A3","scenario":null},{"value":"2,47E-01","module":"A4","scenario":null},{"value":"0,00E+00","module":"C1","scenario":null},{"value":"0,00E+00","module":"C2","scenario":null},{"value":"0,00E+00","module":"C3","scenario":null},{"value":"0,00E+00","module":"C4","scenario":null},{"value":"0,00E+00","module":"D","scenario":null}]},{"parameter":"WDP","unit":"m3 world-eq. Deprived","values":[{"value":"3,69E+00","module":"A1-A3","scenario":null},{"value":"2,39E-01","module":"A4","scenario":null},{"value":"0,00E+00","module":"C1","scenario":null},{"value":"0,00E+00","module":"C2","scenario":null},{"value":"0,00E+00","module":"C3","scenario":null},{"value":"0,00E+00","module":"C4","scenario":null},{"value":"0,00E+00","module":"D","scenario":null}]},{"parameter":"EP-freshwater","unit":"kg P-eq","values":[{"value":"9,15E-06","module":"A1-A3","scenario":null},{"value":"1,31E-07","module":"A4","scenario":null},{"value":"0,00E+00","module":"C1","scenario":null},{"value":"0,00E+00","module":"C2","scenario":null},{"value":"0,00E+00","module":"C3","scenario":null},{"value":"0,00E+00","module":"C4","scenario":null},{"value":"0,00E+00","module":"D","scenario":null}]},{"parameter":"EP-marine","unit":"kg N-eq","values":[{"value":"3,04E-03","module":"A1-A3","scenario":null},{"value":"9,29E-06","module":"A4","scenario":null},{"value":"0,00E+00","module":"C1","scenario":null},{"value":"0,00E+00","module":"C2","scenario":null},{"value":"0,00E+00","module":"C3","scenario":null},{"value":"0,00E+00","module":"C4","scenario":null},{"value":"0,00E+00","module":"D","scenario":null}]},{"parameter":"EP-terrestrial","unit":"mol N-eq.","values":[{"value":"3,19E-02","module":"A1-A3","scenario":null},{"value":"1,04E-04","module":"A4","scenario":null},{"value":"0,00E+00","module":"C1","scenario":null},{"value":"0,00E+00","module":"C2","scenario":null},{"value":"0,00E+00","module":"C3","scenario":null},{"value":"0,00E+00","module":"C4","scenario":null},{"value":"0,00E+00","module":"D","scenario":null}]},{"parameter":"GWP-IOBC","unit":"kg CO2-eq","values":[{"value":"3,88E+00","module":"A1-A3","scenario":null},{"value":"1,63E-02","module":"A4","scenario":null},{"value":"0,00E+00","module":"C1","scenario":null},{"value":"0,00E+00","module":"C2","scenario":null},{"value":"0,00E+00","module":"C3","scenario":null},{"value":"0,00E+00","module":"C4","scenario":null},{"value":"0,00E+00","module":"D","scenario":null}]}],"additional_environmental_impact":[{"parameter":"PM","unit":"Disease incidence","values":[{"value":"1,00E-08","module":"A1-A3","scenario":null},{"value":"1,00E-09","module":"A4","scenario":null},{"value":"0,00E+00","module":"C1","scenario":null},{"value":"0,00E+00","module":"C2","scenario":null},{"value":"0,00E+00","module":"C3","scenario":null},{"value":"0,00E+00","module":"C4","scenario":null},{"value":"0,00E+00","module":"D","scenario":null}]},{"parameter":"ETP-fw","unit":"CTUe","values":[{"value":"1,83E+00","module":"A1-A3","scenario":null},{"value":"1,83E-01","module":"A4","scenario":null},{"value":"0,00E+00","module":"C1","scenario":null},{"value":"0,00E+00","module":"C2","scenario":null},{"value":"0,00E+00","module":"C3","scenario":null},{"value":"0,00E+00","module":"C4","scenario":null},{"value":"0,00E+00","module":"D","scenario":null}]},{"parameter":"HTP-c","unit":"CTUh","values":[{"value":"0,00E+00","module":"A1-A3","scenario":null},{"value":"0,00E+00","module":"A4","scenario":null},{"value":"0,00E+00","module":"C1","scenario":null},{"value":"0,00E+00","module":"C2","scenario":null},{"value":"0,00E+00","module":"C3","scenario":null},{"value":"0,00E+00","module":"C4","scenario":null},{"value":"0,00E+00","module":"D","scenario":null}]},{"parameter":"HTP-nc","unit":"CTUh","values":[{"value":"2,00E-09","module":"A1-A3","scenario":null},{"value":"2,00E-10","module":"A4","scenario":null},{"value":"0,00E+00","module":"C1","scenario":null},{"value":"0,00E+00","module":"C2","scenario":null},{"value":"0,00E+00","module":"C3","scenario":null},{"value":"0,00E+00","module":"C4","scenario":null},{"value":"0,00E+00","module":"D","scenario":null}]},{"parameter":"SQP","unit":"-","values":[{"value":"1,73E+00","module":"A1-A3","scenario":null},{"value":"1,73E-01","module":"A4","scenario":null},{"value":"0,00E+00","module":"C1","scenario":null},{"value":"0,00E+00","module":"C2","scenario":null},{"value":"0,00E+00","module":"C3","scenario":null},{"value":"0,00E+00","module":"C4","scenario":null},{"value":"0,00E+00","module":"D","scenario":null}]},{"parameter":"IRP","unit":"kBq U235-eq","values":[{"value":"1,08E-02","module":"A1-A3","scenario":null},{"value":"1,08E-03","module":"A4","scenario":null},{"value":"0,00E+00","module":"C1","scenario":null},{"value":"0,00E+00","module":"C2","scenario":null},{"value":"0,00E+00","module":"C3","scenario":null},{"value":"0,00E+00","module":"C4","scenario":null},{"value":"0,00E+00","module":"D","scenario":null}]}],"resource_use":[{"parameter":"PERE","unit":"MJ","values":[{"value":"1,09E+01","module":"A1-A3","scenario":null},{"value":"3,54E-03","module":"A4","scenario":null},{"value":"0,00E+00","module":"C1","scenario":null},{"value":"0,00E+00","module":"C2","scenario":null},{"value":"0,00E+00","module":"C3","scenario":null},{"value":"0,00E+00","module":"C4","scenario":null},{"value":"0,00E+00","module":"D","scenario":null}]},{"parameter":"PERM","unit":"","values":[{"value":"0,00E+00","module":"A1-A3","scenario":null},{"value":"0,00E+00","module":"A4","scenario":null},{"value":"0,00E+00","module":"C1","scenario":null},{"value":"0,00E+00","module":"C2","scenario":null},{"value":"0,00E+00","module":"C3","scenario":null},{"value":"0,00E+00","module":"C4","scenario":null},{"value":"0,00E+00","module":"D","scenario":null}]},{"parameter":"PERT","unit":"MJ","values":[{"value":"1,09E+01","module":"A1-A3","scenario":null},{"value":"3,54E-03","module":"A4","scenario":null},{"value":"0,00E+00","module":"C1","scenario":null},{"value":"0,00E+00","module":"C2","scenario":null},{"value":"0,00E+00","module":"C3","scenario":null},{"value":"0,00E+00","module":"C4","scenario":null},{"value":"0,00E+00","module":"D","scenario":null}]},{"parameter":"PENRE","unit":"MJ","values":[{"value":"5,25E+01","module":"A1-A3","scenario":null},{"value":"2,47E-01","module":"A4","scenario":null},{"value":"0,00E+00","module":"C1","scenario":null},{"value":"0,00E+00","module":"C2","scenario":null},{"value":"0,00E+00","module":"C3","scenario":null},{"value":"0,00E+00","module":"C4","scenario":null},{"value":"0,00E+00","module":"D","scenario":null}]},{"parameter":"PENRM","unit":"MJ","values":[{"value":"1,03E+01","module":"A1-A3","scenario":null},{"value":"0,00E+00","module":"A4","scenario":null},{"value":"0,00E+00","module":"C1","scenario":null},{"value":"0,00E+00","module":"C2","scenario":null},{"value":"0,00E+00","module":"C3","scenario":null},{"value":"0,00E+00","module":"C4","scenario":null},{"value":"0,00E+00","module":"D","scenario":null}]},{"parameter":"PENRT","unit":"MJ","values":[{"value":"6,28E+01","module":"A1-A3","scenario":null},{"value":"2,47E-01","module":"A4","scenario":null},{"value":"0,00E+00","module":"C1","scenario":null},{"value":"0,00E+00","module":"C2","scenario":null},{"value":"0,00E+00","module":"C3","scenario":null},{"value":"0,00E+00","module":"C4","scenario":null},{"value":"0,00E+00","module":"D","scenario":null}]},{"parameter":"SM","unit":"kg","values":[{"value":"0,00E+00","module":"A1-A3","scenario":null},{"value":"0,00E+00","module":"A4","scenario":null},{"value":"0,00E+00","module":"C1","scenario":null},{"value":"0,00E+00","module":"C2","scenario":null},{"value":"0,00E+00","module":"C3","scenario":null},{"value":"0,00E+00","module":"C4","scenario":null},{"value":"0,00E+00","module":"D","scenario":null}]},{"parameter":"RSF","unit":"MJ","values":[{"value":"1,27E-03","module":"A1-A3","scenario":null},{"value":"1,26E-04","module":"A4","scenario":null},{"value":"0,00E+00","module":"C1","scenario":null},{"value":"0,00E+00","module":"C2","scenario":null},{"value":"0,00E+00","module":"C3","scenario":null},{"value":"0,00E+00","module":"C4","scenario":null},{"value":"0,00E+00","module":"D","scenario":null}]},{"parameter":"NRSF","unit":"MJ","values":[{"value":"4,53E-03","module":"A1-A3","scenario":null},{"value":"4,52E-04","module":"A4","scenario":null},{"value":"0,00E+00","module":"C1","scenario":null},{"value":"0,00E+00","module":"C2","scenario":null},{"value":"0,00E+00","module":"C3","scenario":null},{"value":"0,00E+00","module":"C4","scenario":null},{"value":"0,00E+00","module":"D","scenario":null}]},{"parameter":"FW","unit":"m3","values":[{"value":"3,60E-02","module":"A1-A3","scenario":null},{"value":"2,64E-05","module":"A4","scenario":null},{"value":"0,00E+00","module":"C1","scenario":null},{"value":"0,00E+00","module":"C2","scenario":null},{"value":"0,00E+00","module":"C3","scenario":null},{"value":"0,00E+00","module":"C4","scenario":null},{"value":"0,00E+00","module":"D","scenario":null}]}],"end_of_life_waste":[{"parameter":"HWD","unit":"kg","values":[{"value":"1,28E-04","module":"A1-A3","scenario":null},{"value":"1,27E-05","module":"A4","scenario":null},{"value":"0,00E+00","module":"C1","scenario":null},{"value":"0,00E+00","module":"C2","scenario":null},{"value":"0,00E+00","module":"C3","scenario":null},{"value":"0,00E+00","module":"C4","scenario":null},{"value":"0,00E+00","module":"D","scenario":null}]},{"parameter":"NHWD","unit":"kg","values":[{"value":"1,41E-01","module":"A1-A3","scenario":null},{"value":"1,20E-02","module":"A4","scenario":null},{"value":"0,00E+00","module":"C1","scenario":null},{"value":"0,00E+00","module":"C2","scenario":null},{"value":"0,00E+00","module":"C3","scenario":null},{"value":"0,00E+00","module":"C4","scenario":null},{"value":"0,00E+00","module":"D","scenario":null}]},{"parameter":"RWD","unit":"kg","values":[{"value":"1,69E-05","module":"A1-A3","scenario":null},{"value":"1,68E-06","module":"A4","scenario":null},{"value":"0,00E+00","module":"C1","scenario":null},{"value":"0,00E+00","module":"C2","scenario":null},{"value":"0,00E+00","module":"C3","scenario":null},{"value":"0,00E+00","module":"C4","scenario":null},{"value":"0,00E+00","module":"D","scenario":null}]}],"end_of_life_flow":[{"parameter":"CRU","unit":"kg","values":[{"value":"0,00E+00","module":"A1-A3","scenario":null},{"value":"0,00E+00","module":"A4","scenario":null},{"value":"0,00E+00","module":"C1","scenario":null},{"value":"0,00E+00","module":"C2","scenario":null},{"value":"0,00E+00","module":"C3","scenario":null},{"value":"0,00E+00","module":"C4","scenario":null},{"value":"0,00E+00","module":"D","scenario":null}]},{"parameter":"MFR","unit":"kg","values":[{"value":"0,00E+00","module":"A1-A3","scenario":null},{"value":"0,00E+00","module":"A4","scenario":null},{"value":"0,00E+00","module":"C1","scenario":null},{"value":"0,00E+00","module":"C2","scenario":null},{"value":"0,00E+00","module":"C3","scenario":null},{"value":"0,00E+00","module":"C4","scenario":null},{"value":"0,00E+00","module":"D","scenario":null}]},{"parameter":"MER","unit":"kg","values":[{"value":"0,00E+00","module":"A1-A3","scenario":null},{"value":"0,00E+00","module":"A4","scenario":null},{"value":"0,00E+00","module":"C1","scenario":null},{"value":"0,00E+00","module":"C2","scenario":null},{"value":"0,00E+00","module":"C3","scenario":null},{"value":"0,00E+00","module":"C4","scenario":null},{"value":"0,00E+00","module":"D","scenario":null}]},{"parameter":"EEE","unit":"MJ","values":[{"value":"0,00E+00","module":"A1-A3","scenario":null},{"value":"0,00E+00","module":"A4","scenario":null},{"value":"0,00E+00","module":"C1","scenario":null},{"value":"0,00E+00","module":"C2","scenario":null},{"value":"0,00E+00","module":"C3","scenario":null},{"value":"0,00E+00","module":"C4","scenario":null},{"value":"0,00E+00","module":"D","scenario":null}]},{"parameter":"EET","unit":"MJ","values":[{"value":"0,00E+00","module":"A1-A3","scenario":null},{"value":"0,00E+00","module":"A4","scenario":null},{"value":"0,00E+00","module":"C1","scenario":null},{"value":"0,00E+00","module":"C2","scenario":null},{"value":"0,00E+00","module":"C3","scenario":null},{"value":"0,00E+00","module":"C4","scenario":null},{"value":"0,00E+00","module":"D","scenario":null}]}]}