{"product_name":"Component EPD Ringebu: Injection moulded PP fittings and gullies from Surnadal - used as material component in various finished mixed products","epd_id":"NEPD-7772-7150","declared_unit":{"unit":"ton","amount":1},"compliance":["EN 15804+A2","ISO 14025","ISO 21930"],"producer_name":"Pipelife Norge AS","environmental_impact":[{"parameter":"GWP-total","unit":"kg CO2-eq","values":[{"value":"2,84E+00","module":"A1-A3","scenario":null},{"value":"1,63E-02","module":"A4","scenario":null},{"value":"0,00E+00","module":"A5","scenario":null},{"value":"0,00E+00","module":"C1","scenario":null},{"value":"0,00E+00","module":"C2","scenario":null},{"value":"1,27E+00","module":"C3","scenario":null},{"value":"5,79E-02","module":"C4","scenario":null},{"value":"-7,40E-02","module":"D","scenario":null}]},{"parameter":"GWP-fossil","unit":"kg CO2-eq","values":[{"value":"2,82E+00","module":"A1-A3","scenario":null},{"value":"1,63E-02","module":"A4","scenario":null},{"value":"0,00E+00","module":"A5","scenario":null},{"value":"0,00E+00","module":"C1","scenario":null},{"value":"0,00E+00","module":"C2","scenario":null},{"value":"1,27E+00","module":"C3","scenario":null},{"value":"5,79E-02","module":"C4","scenario":null},{"value":"-7,14E-02","module":"D","scenario":null}]},{"parameter":"GWP-biogenic","unit":"kg CO2-eq","values":[{"value":"2,17E-02","module":"A1-A3","scenario":null},{"value":"6,76E-06","module":"A4","scenario":null},{"value":"0,00E+00","module":"A5","scenario":null},{"value":"0,00E+00","module":"C1","scenario":null},{"value":"0,00E+00","module":"C2","scenario":null},{"value":"1,05E-05","module":"C3","scenario":null},{"value":"5,52E-06","module":"C4","scenario":null},{"value":"-1,47E-04","module":"D","scenario":null}]},{"parameter":"GWP-luluc","unit":"kg CO2-eq","values":[{"value":"4,83E-03","module":"A1-A3","scenario":null},{"value":"5,81E-06","module":"A4","scenario":null},{"value":"0,00E+00","module":"A5","scenario":null},{"value":"0,00E+00","module":"C1","scenario":null},{"value":"0,00E+00","module":"C2","scenario":null},{"value":"1,61E-06","module":"C3","scenario":null},{"value":"1,24E-06","module":"C4","scenario":null},{"value":"-2,46E-03","module":"D","scenario":null}]},{"parameter":"ODP","unit":"kg CFC11-eq","values":[{"value":"1,95E-07","module":"A1-A3","scenario":null},{"value":"3,70E-09","module":"A4","scenario":null},{"value":"0,00E+00","module":"A5","scenario":null},{"value":"0,00E+00","module":"C1","scenario":null},{"value":"0,00E+00","module":"C2","scenario":null},{"value":"1,00E-09","module":"C3","scenario":null},{"value":"1,65E-09","module":"C4","scenario":null},{"value":"-5,20E-03","module":"D","scenario":null}]},{"parameter":"AP","unit":"mol H+-eq","values":[{"value":"1,29E-02","module":"A1-A3","scenario":null},{"value":"4,69E-05","module":"A4","scenario":null},{"value":"0,00E+00","module":"A5","scenario":null},{"value":"0,00E+00","module":"C1","scenario":null},{"value":"0,00E+00","module":"C2","scenario":null},{"value":"1,61E-04","module":"C3","scenario":null},{"value":"4,16E-05","module":"C4","scenario":null},{"value":"-5,88E-04","module":"D","scenario":null}]},{"parameter":"POCP","unit":"kg NMVOC-eq","values":[{"value":"1,10E-02","module":"A1-A3","scenario":null},{"value":"3,98E-05","module":"A4","scenario":null},{"value":"0,00E+00","module":"A5","scenario":null},{"value":"0,00E+00","module":"C1","scenario":null},{"value":"0,00E+00","module":"C2","scenario":null},{"value":"2,00E-04","module":"C3","scenario":null},{"value":"5,88E-05","module":"C4","scenario":null},{"value":"-5,73E-04","module":"D","scenario":null}]},{"parameter":"ADPE","unit":"kg Sb-eq","values":[{"value":"1,20E-04","module":"A1-A3","scenario":null},{"value":"4,51E-07","module":"A4","scenario":null},{"value":"0,00E+00","module":"A5","scenario":null},{"value":"0,00E+00","module":"C1","scenario":null},{"value":"0,00E+00","module":"C2","scenario":null},{"value":"4,67E-08","module":"C3","scenario":null},{"value":"4,23E-08","module":"C4","scenario":null},{"value":"-7,10E-07","module":"D","scenario":null}]},{"parameter":"ADPF","unit":"MJ","values":[{"value":"8,43E+01","module":"A1-A3","scenario":null},{"value":"2,47E-01","module":"A4","scenario":null},{"value":"0,00E+00","module":"A5","scenario":null},{"value":"0,00E+00","module":"C1","scenario":null},{"value":"0,00E+00","module":"C2","scenario":null},{"value":"8,63E-02","module":"C3","scenario":null},{"value":"1,22E-01","module":"C4","scenario":null},{"value":"-1,02E+00","module":"D","scenario":null}]},{"parameter":"WDP","unit":"m3 world-eq. Deprived","values":[{"value":"6,47E+02","module":"A1-A3","scenario":null},{"value":"2,39E-01","module":"A4","scenario":null},{"value":"0,00E+00","module":"A5","scenario":null},{"value":"0,00E+00","module":"C1","scenario":null},{"value":"0,00E+00","module":"C2","scenario":null},{"value":"2,01E-01","module":"C3","scenario":null},{"value":"1,05E+00","module":"C4","scenario":null},{"value":"-1,27E+01","module":"D","scenario":null}]},{"parameter":"EP-freshwater","unit":"kg P-eq","values":[{"value":"8,32E-05","module":"A1-A3","scenario":null},{"value":"1,31E-07","module":"A4","scenario":null},{"value":"0,00E+00","module":"A5","scenario":null},{"value":"0,00E+00","module":"C1","scenario":null},{"value":"0,00E+00","module":"C2","scenario":null},{"value":"1,07E-07","module":"C3","scenario":null},{"value":"6,24E-08","module":"C4","scenario":null},{"value":"-6,34E-06","module":"D","scenario":null}]},{"parameter":"EP-marine","unit":"kg N-eq","values":[{"value":"2,56E-03","module":"A1-A3","scenario":null},{"value":"9,29E-06","module":"A4","scenario":null},{"value":"0,00E+00","module":"A5","scenario":null},{"value":"0,00E+00","module":"C1","scenario":null},{"value":"0,00E+00","module":"C2","scenario":null},{"value":"7,68E-05","module":"C3","scenario":null},{"value":"7,41E-05","module":"C4","scenario":null},{"value":"-1,92E-04","module":"D","scenario":null}]},{"parameter":"EP-terrestrial","unit":"mol N-eq.","values":[{"value":"2,83E-02","module":"A1-A3","scenario":null},{"value":"1,04E-04","module":"A4","scenario":null},{"value":"0,00E+00","module":"A5","scenario":null},{"value":"0,00E+00","module":"C1","scenario":null},{"value":"0,00E+00","module":"C2","scenario":null},{"value":"8,31E-04","module":"C3","scenario":null},{"value":"1,64E-04","module":"C4","scenario":null},{"value":"-2,08E-03","module":"D","scenario":null}]},{"parameter":"GWP-IOBC","unit":"kg CO2-eq","values":[{"value":"2,74E+00","module":"A1-A3","scenario":null},{"value":"1,63E-02","module":"A4","scenario":null},{"value":"0,00E+00","module":"A5","scenario":null},{"value":"0,00E+00","module":"C1","scenario":null},{"value":"0,00E+00","module":"C2","scenario":null},{"value":"1,27E+00","module":"C3","scenario":null},{"value":"5,80E-02","module":"C4","scenario":null},{"value":"-7,29E-02","module":"D","scenario":null}]}],"additional_environmental_impact":[{"parameter":"PM","unit":"Disease incidence","values":[{"value":"1,40E-07","module":"A1-A3","scenario":null},{"value":"1,00E-09","module":"A4","scenario":null},{"value":"0,00E+00","module":"A5","scenario":null},{"value":"0,00E+00","module":"C1","scenario":null},{"value":"0,00E+00","module":"C2","scenario":null},{"value":"7,52E-10","module":"C3","scenario":null},{"value":"8,18E-10","module":"C4","scenario":null},{"value":"-3,56E-08","module":"D","scenario":null}]},{"parameter":"ETP-fw","unit":"CTUe","values":[{"value":"5,31E+01","module":"A1-A3","scenario":null},{"value":"1,83E-01","module":"A4","scenario":null},{"value":"0,00E+00","module":"A5","scenario":null},{"value":"0,00E+00","module":"C1","scenario":null},{"value":"0,00E+00","module":"C2","scenario":null},{"value":"2,55E-01","module":"C3","scenario":null},{"value":"1,52E-01","module":"C4","scenario":null},{"value":"-5,55E+00","module":"D","scenario":null}]},{"parameter":"HTP-c","unit":"CTUh","values":[{"value":"1,42E-09","module":"A1-A3","scenario":null},{"value":"0,00E+00","module":"A4","scenario":null},{"value":"0,00E+00","module":"A5","scenario":null},{"value":"0,00E+00","module":"C1","scenario":null},{"value":"0,00E+00","module":"C2","scenario":null},{"value":"3,00E-11","module":"C3","scenario":null},{"value":"4,00E-12","module":"C4","scenario":null},{"value":"-1,01E-10","module":"D","scenario":null}]},{"parameter":"HTP-nc","unit":"CTUh","values":[{"value":"3,68E-08","module":"A1-A3","scenario":null},{"value":"2,00E-10","module":"A4","scenario":null},{"value":"0,00E+00","module":"A5","scenario":null},{"value":"0,00E+00","module":"C1","scenario":null},{"value":"0,00E+00","module":"C2","scenario":null},{"value":"1,09E-09","module":"C3","scenario":null},{"value":"1,14E-10","module":"C4","scenario":null},{"value":"-5,32E-09","module":"D","scenario":null}]},{"parameter":"SQP","unit":"-","values":[{"value":"4,64E+01","module":"A1-A3","scenario":null},{"value":"1,73E-01","module":"A4","scenario":null},{"value":"0,00E+00","module":"A5","scenario":null},{"value":"0,00E+00","module":"C1","scenario":null},{"value":"0,00E+00","module":"C2","scenario":null},{"value":"1,09E-02","module":"C3","scenario":null},{"value":"4,55E-01","module":"C4","scenario":null},{"value":"-6,83E+00","module":"D","scenario":null}]},{"parameter":"IRP","unit":"kBq U235-eq","values":[{"value":"1,48E-01","module":"A1-A3","scenario":null},{"value":"1,08E-03","module":"A4","scenario":null},{"value":"0,00E+00","module":"A5","scenario":null},{"value":"0,00E+00","module":"C1","scenario":null},{"value":"0,00E+00","module":"C2","scenario":null},{"value":"1,50E-04","module":"C3","scenario":null},{"value":"5,90E-04","module":"C4","scenario":null},{"value":"-6,52E-03","module":"D","scenario":null}]}],"resource_use":[{"parameter":"PERE","unit":"MJ","values":[{"value":"5,01E+01","module":"A1-A3","scenario":null},{"value":"3,54E-03","module":"A4","scenario":null},{"value":"0,00E+00","module":"A5","scenario":null},{"value":"0,00E+00","module":"C1","scenario":null},{"value":"0,00E+00","module":"C2","scenario":null},{"value":"2,62E-03","module":"C3","scenario":null},{"value":"5,75E-03","module":"C4","scenario":null},{"value":"-6,31E+00","module":"D","scenario":null}]},{"parameter":"PERM","unit":"","values":[{"value":"0,00E+00","module":"A1-A3","scenario":null},{"value":"0,00E+00","module":"A4","scenario":null},{"value":"0,00E+00","module":"A5","scenario":null},{"value":"0,00E+00","module":"C1","scenario":null},{"value":"0,00E+00","module":"C2","scenario":null},{"value":"0,00E+00","module":"C3","scenario":null},{"value":"0,00E+00","module":"C4","scenario":null},{"value":"0,00E+00","module":"D","scenario":null}]},{"parameter":"PERT","unit":"MJ","values":[{"value":"5,01E+01","module":"A1-A3","scenario":null},{"value":"3,54E-03","module":"A4","scenario":null},{"value":"0,00E+00","module":"A5","scenario":null},{"value":"0,00E+00","module":"C1","scenario":null},{"value":"0,00E+00","module":"C2","scenario":null},{"value":"2,62E-03","module":"C3","scenario":null},{"value":"5,75E-03","module":"C4","scenario":null},{"value":"-6,31E+00","module":"D","scenario":null}]},{"parameter":"PENRE","unit":"MJ","values":[{"value":"5,41E+01","module":"A1-A3","scenario":null},{"value":"2,47E-01","module":"A4","scenario":null},{"value":"0,00E+00","module":"A5","scenario":null},{"value":"0,00E+00","module":"C1","scenario":null},{"value":"0,00E+00","module":"C2","scenario":null},{"value":"8,63E-02","module":"C3","scenario":null},{"value":"1,22E-01","module":"C4","scenario":null},{"value":"-1,02E+00","module":"D","scenario":null}]},{"parameter":"PENRM","unit":"MJ","values":[{"value":"3,26E+01","module":"A1-A3","scenario":null},{"value":"0,00E+00","module":"A4","scenario":null},{"value":"0,00E+00","module":"A5","scenario":null},{"value":"0,00E+00","module":"C1","scenario":null},{"value":"0,00E+00","module":"C2","scenario":null},{"value":"-3,26E+01","module":"C3","scenario":null},{"value":"0,00E+00","module":"C4","scenario":null},{"value":"0,00E+00","module":"D","scenario":null}]},{"parameter":"PENRT","unit":"MJ","values":[{"value":"8,67E+01","module":"A1-A3","scenario":null},{"value":"2,47E-01","module":"A4","scenario":null},{"value":"0,00E+00","module":"A5","scenario":null},{"value":"0,00E+00","module":"C1","scenario":null},{"value":"0,00E+00","module":"C2","scenario":null},{"value":"-3,25E+01","module":"C3","scenario":null},{"value":"1,22E-01","module":"C4","scenario":null},{"value":"-1,02E+00","module":"D","scenario":null}]},{"parameter":"SM","unit":"kg","values":[{"value":"0,00E+00","module":"A1-A3","scenario":null},{"value":"0,00E+00","module":"A4","scenario":null},{"value":"0,00E+00","module":"A5","scenario":null},{"value":"0,00E+00","module":"C1","scenario":null},{"value":"0,00E+00","module":"C2","scenario":null},{"value":"0,00E+00","module":"C3","scenario":null},{"value":"0,00E+00","module":"C4","scenario":null},{"value":"0,00E+00","module":"D","scenario":null}]},{"parameter":"RSF","unit":"MJ","values":[{"value":"1,25E-01","module":"A1-A3","scenario":null},{"value":"1,26E-04","module":"A4","scenario":null},{"value":"0,00E+00","module":"A5","scenario":null},{"value":"0,00E+00","module":"C1","scenario":null},{"value":"0,00E+00","module":"C2","scenario":null},{"value":"7,21E-05","module":"C3","scenario":null},{"value":"1,21E-04","module":"C4","scenario":null},{"value":"-1,10E-03","module":"D","scenario":null}]},{"parameter":"NRSF","unit":"MJ","values":[{"value":"9,97E-02","module":"A1-A3","scenario":null},{"value":"4,52E-04","module":"A4","scenario":null},{"value":"0,00E+00","module":"A5","scenario":null},{"value":"0,00E+00","module":"C1","scenario":null},{"value":"0,00E+00","module":"C2","scenario":null},{"value":"0,00E+00","module":"C3","scenario":null},{"value":"1,97E-03","module":"C4","scenario":null},{"value":"-3,74E-01","module":"D","scenario":null}]},{"parameter":"FW","unit":"m3","values":[{"value":"3,47E-01","module":"A1-A3","scenario":null},{"value":"2,64E-05","module":"A4","scenario":null},{"value":"0,00E+00","module":"A5","scenario":null},{"value":"0,00E+00","module":"C1","scenario":null},{"value":"0,00E+00","module":"C2","scenario":null},{"value":"2,38E-04","module":"C3","scenario":null},{"value":"1,50E-04","module":"C4","scenario":null},{"value":"-7,59E-03","module":"D","scenario":null}]}],"end_of_life_waste":[{"parameter":"HWD","unit":"kg","values":[{"value":"7,90E-03","module":"A1-A3","scenario":null},{"value":"1,27E-05","module":"A4","scenario":null},{"value":"0,00E+00","module":"A5","scenario":null},{"value":"0,00E+00","module":"C1","scenario":null},{"value":"0,00E+00","module":"C2","scenario":null},{"value":"0,00E+00","module":"C3","scenario":null},{"value":"1,26E-02","module":"C4","scenario":null},{"value":"-4,80E-05","module":"D","scenario":null}]},{"parameter":"NHWD","unit":"kg","values":[{"value":"4,62E-01","module":"A1-A3","scenario":null},{"value":"1,20E-02","module":"A4","scenario":null},{"value":"0,00E+00","module":"A5","scenario":null},{"value":"0,00E+00","module":"C1","scenario":null},{"value":"0,00E+00","module":"C2","scenario":null},{"value":"0,00E+00","module":"C3","scenario":null},{"value":"5,07E-01","module":"C4","scenario":null},{"value":"-2,41E-02","module":"D","scenario":null}]},{"parameter":"RWD","unit":"kg","values":[{"value":"1,29E-04","module":"A1-A3","scenario":null},{"value":"1,68E-06","module":"A4","scenario":null},{"value":"0,00E+00","module":"A5","scenario":null},{"value":"0,00E+00","module":"C1","scenario":null},{"value":"0,00E+00","module":"C2","scenario":null},{"value":"0,00E+00","module":"C3","scenario":null},{"value":"8,02E-07","module":"C4","scenario":null},{"value":"-5,34E-06","module":"D","scenario":null}]}],"end_of_life_flow":[{"parameter":"CRU","unit":"kg","values":[{"value":"0,00E+00","module":"A1-A3","scenario":null},{"value":"0,00E+00","module":"A4","scenario":null},{"value":"0,00E+00","module":"A5","scenario":null},{"value":"0,00E+00","module":"C1","scenario":null},{"value":"0,00E+00","module":"C2","scenario":null},{"value":"0,00E+00","module":"C3","scenario":null},{"value":"0,00E+00","module":"C4","scenario":null},{"value":"0,00E+00","module":"D","scenario":null}]},{"parameter":"MFR","unit":"kg","values":[{"value":"0,00E+00","module":"A1-A3","scenario":null},{"value":"0,00E+00","module":"A4","scenario":null},{"value":"0,00E+00","module":"A5","scenario":null},{"value":"0,00E+00","module":"C1","scenario":null},{"value":"0,00E+00","module":"C2","scenario":null},{"value":"0,00E+00","module":"C3","scenario":null},{"value":"4,48E-05","module":"C4","scenario":null},{"value":"0,00E+00","module":"D","scenario":null}]},{"parameter":"MER","unit":"kg","values":[{"value":"0,00E+00","module":"A1-A3","scenario":null},{"value":"0,00E+00","module":"A4","scenario":null},{"value":"0,00E+00","module":"A5","scenario":null},{"value":"0,00E+00","module":"C1","scenario":null},{"value":"0,00E+00","module":"C2","scenario":null},{"value":"5,00E-01","module":"C3","scenario":null},{"value":"1,10E-06","module":"C4","scenario":null},{"value":"0,00E+00","module":"D","scenario":null}]},{"parameter":"EEE","unit":"MJ","values":[{"value":"0,00E+00","module":"A1-A3","scenario":null},{"value":"0,00E+00","module":"A4","scenario":null},{"value":"0,00E+00","module":"A5","scenario":null},{"value":"0,00E+00","module":"C1","scenario":null},{"value":"0,00E+00","module":"C2","scenario":null},{"value":"8,14E-01","module":"C3","scenario":null},{"value":"7,12E-05","module":"C4","scenario":null},{"value":"0,00E+00","module":"D","scenario":null}]},{"parameter":"EET","unit":"MJ","values":[{"value":"0,00E+00","module":"A1-A3","scenario":null},{"value":"0,00E+00","module":"A4","scenario":null},{"value":"0,00E+00","module":"A5","scenario":null},{"value":"0,00E+00","module":"C1","scenario":null},{"value":"0,00E+00","module":"C2","scenario":null},{"value":"1,23E+01","module":"C3","scenario":null},{"value":"1,08E-03","module":"C4","scenario":null},{"value":"0,00E+00","module":"D","scenario":null}]}]}