{"product_name":"IRIS cabinet with variants (IRIS High cabinet 5A4,  2A4 doors lower, 3A4 glass doors upper, meas. w/o base 2100x1000x600, melamine)","epd_id":"NEPD-6278-5542-EN","compliance":["EN 15804+A2","ISO 14025","ISO 21930"],"producer_name":"Svenheim M\u00f8belindustri AS","environmental_impact":[{"parameter":"GWP-total","unit":"kg CO2-eq.","values":[{"value":"-8,49E+01","module":"A1-A3"},{"value":"3,00E+01","module":"A4"},{"value":"0,0E+00","module":"A5"},{"value":"0,0E+00","module":"C1"},{"value":"1,63E+00","module":"C2"},{"value":"1,82E+02","module":"C3"},{"value":"1,56E-01","module":"C4"},{"value":"-7,55E+00","module":"D"}]},{"parameter":"GWP-fossil","unit":"kg CO2-eq.","values":[{"value":"1,19E+02","module":"A1-A3"},{"value":"3,00E+01","module":"A4"},{"value":"0,0E+00","module":"A5"},{"value":"0,0E+00","module":"C1"},{"value":"1,63E+00","module":"C2"},{"value":"5,57E+00","module":"C3"},{"value":"1,56E-01","module":"C4"},{"value":"-7,30E+00","module":"D"}]},{"parameter":"GWP-biogenic","unit":"kg CO2-eq.","values":[{"value":"-2,05E+02","module":"A1-A3"},{"value":"1,34E-02","module":"A4"},{"value":"0,0E+00","module":"A5"},{"value":"0,0E+00","module":"C1"},{"value":"6,74E-04","module":"C2"},{"value":"1,76E+02","module":"C3"},{"value":"1,03E-04","module":"C4"},{"value":"-1,49E-02","module":"D"}]},{"parameter":"GWP-luluc","unit":"kg CO2-eq.","values":[{"value":"2,28E-01","module":"A1-A3"},{"value":"1,47E-02","module":"A4"},{"value":"0,0E+00","module":"A5"},{"value":"0,0E+00","module":"C1"},{"value":"5,79E-04","module":"C2"},{"value":"3,29E-04","module":"C3"},{"value":"3,83E-05","module":"C4"},{"value":"-2,40E-01","module":"D"}]},{"parameter":"ODP","unit":"kg CFC 11-eq.","values":[{"value":"1,44E-05","module":"A1-A3"},{"value":"6,64E-06","module":"A4"},{"value":"0,0E+00","module":"A5"},{"value":"0,0E+00","module":"C1"},{"value":"3,69E-07","module":"C2"},{"value":"1,62E-07","module":"C3"},{"value":"3,66E-08","module":"C4"},{"value":"-5,04E-01","module":"D"}]},{"parameter":"AP","unit":"mol H+-eq.","values":[{"value":"8,06E-01","module":"A1-A3"},{"value":"1,05E-01","module":"A4"},{"value":"0,0E+00","module":"A5"},{"value":"0,0E+00","module":"C1"},{"value":"4,68E-03","module":"C2"},{"value":"1,74E-02","module":"C3"},{"value":"8,93E-04","module":"C4"},{"value":"-5,90E-02","module":"D"}]},{"parameter":"POCP","unit":"kg NMVOC-eq.","values":[{"value":"6,06E-01","module":"A1-A3"},{"value":"9,94E-02","module":"A4"},{"value":"0,0E+00","module":"A5"},{"value":"0,0E+00","module":"C1"},{"value":"3,96E-03","module":"C2"},{"value":"2,14E-02","module":"C3"},{"value":"9,84E-04","module":"C4"},{"value":"-5,73E-02","module":"D"}]},{"parameter":"ADPE","unit":"kg Sb-eq.","values":[{"value":"2,03E-03","module":"A1-A3"},{"value":"7,77E-04","module":"A4"},{"value":"0,0E+00","module":"A5"},{"value":"0,0E+00","module":"C1"},{"value":"4,49E-05","module":"C2"},{"value":"7,26E-06","module":"C3"},{"value":"2,01E-06","module":"C4"},{"value":"-7,37E-05","module":"D"}]},{"parameter":"ADPF","unit":"MJ","values":[{"value":"2,13E+03","module":"A1-A3"},{"value":"4,47E+02","module":"A4"},{"value":"0,0E+00","module":"A5"},{"value":"0,0E+00","module":"C1"},{"value":"2,46E+01","module":"C2"},{"value":"1,22E+01","module":"C3"},{"value":"2,77E+00","module":"C4"},{"value":"-1,03E+02","module":"D"}]},{"parameter":"WDP","unit":"m3 world-eq.","values":[{"value":"1,36E+04","module":"A1-A3"},{"value":"4,55E+02","module":"A4"},{"value":"0,0E+00","module":"A5"},{"value":"0,0E+00","module":"C1"},{"value":"2,38E+01","module":"C2"},{"value":"1,78E+01","module":"C3"},{"value":"9,99E+00","module":"C4"},{"value":"-1,27E+03","module":"D"}]},{"parameter":"EP-freshwater","unit":"kg P-eq.","values":[{"value":"6,54E-03","module":"A1-A3"},{"value":"2,52E-04","module":"A4"},{"value":"0,0E+00","module":"A5"},{"value":"0,0E+00","module":"C1"},{"value":"1,30E-05","module":"C2"},{"value":"3,04E-05","module":"C3"},{"value":"1,72E-06","module":"C4"},{"value":"-6,36E-04","module":"D"}]},{"parameter":"EP-marine","unit":"kg N-eq.","values":[{"value":"1,43E-01","module":"A1-A3"},{"value":"2,71E-02","module":"A4"},{"value":"0,0E+00","module":"A5"},{"value":"0,0E+00","module":"C1"},{"value":"9,25E-04","module":"C2"},{"value":"8,18E-03","module":"C3"},{"value":"3,09E-04","module":"C4"},{"value":"-1,90E-02","module":"D"}]},{"parameter":"EP-terrestrial","unit":"mol N-eq.","values":[{"value":"2,04E+00","module":"A1-A3"},{"value":"3,01E-01","module":"A4"},{"value":"0,0E+00","module":"A5"},{"value":"0,0E+00","module":"C1"},{"value":"1,04E-02","module":"C2"},{"value":"8,68E-02","module":"C3"},{"value":"3,44E-03","module":"C4"},{"value":"-2,05E-01","module":"D"}]},{"parameter":"GWP-IOBC","unit":"kg CO2-eq.","values":[{"value":"1,55E+02","module":"A1-A3"},{"value":"3,00E+01","module":"A4"},{"value":"0,0E+00","module":"A5"},{"value":"0,0E+00","module":"C1"},{"value":"1,63E+00","module":"C2"},{"value":"3,72E+00","module":"C3"},{"value":"1,61E-01","module":"C4"},{"value":"-7,59E+00","module":"D"}]}],"additional_environmental_impact":[{"parameter":"PM","unit":"disease incidence","values":[{"value":"1,86E-05","module":"A1-A3"},{"value":"1,73E-06","module":"A4"},{"value":"0,0E+00","module":"A5"},{"value":"0,0E+00","module":"C1"},{"value":"9,96E-08","module":"C2"},{"value":"1,94E-07","module":"C3"},{"value":"1,52E-08","module":"C4"},{"value":"-3,48E-06","module":"D"}]},{"parameter":"ETP-fw","unit":"CTUe","values":[{"value":"3,06E+03","module":"A1-A3"},{"value":"3,32E+02","module":"A4"},{"value":"0,0E+00","module":"A5"},{"value":"0,0E+00","module":"C1"},{"value":"1,82E+01","module":"C2"},{"value":"3,73E+01","module":"C3"},{"value":"2,27E+00","module":"C4"},{"value":"-5,56E+02","module":"D"}]},{"parameter":"HTP-c","unit":"CTUh","values":[{"value":"4,70E-07","module":"A1-A3"},{"value":"0,0E+00","module":"A4"},{"value":"0,0E+00","module":"A5"},{"value":"0,0E+00","module":"C1"},{"value":"0,0E+00","module":"C2"},{"value":"4,39E-09","module":"C3"},{"value":"9,50E-11","module":"C4"},{"value":"-1,15E-08","module":"D"}]},{"parameter":"HTP-nc","unit":"CTUh","values":[{"value":"1,89E-06","module":"A1-A3"},{"value":"3,34E-07","module":"A4"},{"value":"0,0E+00","module":"A5"},{"value":"0,0E+00","module":"C1"},{"value":"1,99E-08","module":"C2"},{"value":"1,90E-07","module":"C3"},{"value":"3,01E-09","module":"C4"},{"value":"-4,88E-07","module":"D"}]},{"parameter":"SQP","unit":"unitless","values":[{"value":"9,22E+03","module":"A1-A3"},{"value":"3,16E+02","module":"A4"},{"value":"0,0E+00","module":"A5"},{"value":"0,0E+00","module":"C1"},{"value":"1,72E+01","module":"C2"},{"value":"2,11E+00","module":"C3"},{"value":"6,51E+00","module":"C4"},{"value":"-6,62E+02","module":"D"}]},{"parameter":"IRP","unit":"kBq U235-eq.","values":[{"value":"9,56E+00","module":"A1-A3"},{"value":"1,96E+00","module":"A4"},{"value":"0,0E+00","module":"A5"},{"value":"0,0E+00","module":"C1"},{"value":"1,08E-01","module":"C2"},{"value":"2,78E-02","module":"C3"},{"value":"1,15E-02","module":"C4"},{"value":"-6,36E-01","module":"D"}]}],"resource_use":[{"parameter":"PERE","unit":"MJ","values":[{"value":"1,06E+03","module":"A1-A3"},{"value":"6,80E+00","module":"A4"},{"value":"0,0E+00","module":"A5"},{"value":"0,0E+00","module":"C1"},{"value":"3,52E-01","module":"C2"},{"value":"5,89E-01","module":"C3"},{"value":"7,25E-02","module":"C4"},{"value":"-6,12E+02","module":"D"}]},{"parameter":"PERM","unit":"MJ","values":[{"value":"1,07E+03","module":"A1-A3"},{"value":"0,0E+00","module":"A4"},{"value":"0,0E+00","module":"A5"},{"value":"0,0E+00","module":"C1"},{"value":"0,0E+00","module":"C2"},{"value":"-9,10E+02","module":"C3"},{"value":"0,0E+00","module":"C4"},{"value":"0,0E+00","module":"D"}]},{"parameter":"PERT","unit":"MJ","values":[{"value":"2,12E+03","module":"A1-A3"},{"value":"6,80E+00","module":"A4"},{"value":"0,0E+00","module":"A5"},{"value":"0,0E+00","module":"C1"},{"value":"3,52E-01","module":"C2"},{"value":"-9,10E+02","module":"C3"},{"value":"7,25E-02","module":"C4"},{"value":"-6,12E+02","module":"D"}]},{"parameter":"PENRE","unit":"MJ","values":[{"value":"2,10E+03","module":"A1-A3"},{"value":"4,47E+02","module":"A4"},{"value":"0,0E+00","module":"A5"},{"value":"0,0E+00","module":"C1"},{"value":"2,46E+01","module":"C2"},{"value":"1,24E+01","module":"C3"},{"value":"2,77E+00","module":"C4"},{"value":"-1,03E+02","module":"D"}]},{"parameter":"PENRM","unit":"MJ","values":[{"value":"4,22E+01","module":"A1-A3"},{"value":"0,0E+00","module":"A4"},{"value":"0,0E+00","module":"A5"},{"value":"0,0E+00","module":"C1"},{"value":"0,0E+00","module":"C2"},{"value":"-4,54E+00","module":"C3"},{"value":"0,0E+00","module":"C4"},{"value":"0,0E+00","module":"D"}]},{"parameter":"PENRT","unit":"MJ","values":[{"value":"2,14E+03","module":"A1-A3"},{"value":"4,47E+02","module":"A4"},{"value":"0,0E+00","module":"A5"},{"value":"0,0E+00","module":"C1"},{"value":"2,46E+01","module":"C2"},{"value":"7,82E+00","module":"C3"},{"value":"2,77E+00","module":"C4"},{"value":"-1,03E+02","module":"D"}]},{"parameter":"SM","unit":"kg","values":[{"value":"9,27E-01","module":"A1-A3"},{"value":"0,0E+00","module":"A4"},{"value":"0,0E+00","module":"A5"},{"value":"0,0E+00","module":"C1"},{"value":"0,0E+00","module":"C2"},{"value":"0,0E+00","module":"C3"},{"value":"0,0E+00","module":"C4"},{"value":"0,0E+00","module":"D"}]},{"parameter":"RSF","unit":"MJ","values":[{"value":"1,18E+01","module":"A1-A3"},{"value":"2,67E-01","module":"A4"},{"value":"0,0E+00","module":"A5"},{"value":"0,0E+00","module":"C1"},{"value":"1,26E-02","module":"C2"},{"value":"1,35E-02","module":"C3"},{"value":"1,84E-03","module":"C4"},{"value":"-9,67E-02","module":"D"}]},{"parameter":"NRSF","unit":"MJ","values":[{"value":"2,39E+00","module":"A1-A3"},{"value":"8,86E-01","module":"A4"},{"value":"0,0E+00","module":"A5"},{"value":"0,0E+00","module":"C1"},{"value":"4,51E-02","module":"C2"},{"value":"0,0E+00","module":"C3"},{"value":"4,27E-01","module":"C4"},{"value":"-3,59E+01","module":"D"}]},{"parameter":"FW","unit":"m3","values":[{"value":"2,75E+00","module":"A1-A3"},{"value":"5,05E-02","module":"A4"},{"value":"0,0E+00","module":"A5"},{"value":"0,0E+00","module":"C1"},{"value":"2,63E-03","module":"C2"},{"value":"2,37E-02","module":"C3"},{"value":"2,54E-03","module":"C4"},{"value":"-7,39E-01","module":"D"}]}],"end_of_life_waste":[{"parameter":"HWD","unit":"kg","values":[{"value":"1,12E+00","module":"A1-A3"},{"value":"2,35E-02","module":"A4"},{"value":"0,0E+00","module":"A5"},{"value":"0,0E+00","module":"C1"},{"value":"1,27E-03","module":"C2"},{"value":"0,0E+00","module":"C3"},{"value":"9,81E+00","module":"C4"},{"value":"-5,77E-03","module":"D"}]},{"parameter":"NHWD","unit":"kg","values":[{"value":"1,81E+01","module":"A1-A3"},{"value":"2,02E+01","module":"A4"},{"value":"0,0E+00","module":"A5"},{"value":"0,0E+00","module":"C1"},{"value":"1,20E+00","module":"C2"},{"value":"9,76E+00","module":"C3"},{"value":"4,76E-01","module":"C4"},{"value":"-2,48E+00","module":"D"}]},{"parameter":"RWD","unit":"kg","values":[{"value":"9,18E-03","module":"A1-A3"},{"value":"3,04E-03","module":"A4"},{"value":"0,0E+00","module":"A5"},{"value":"0,0E+00","module":"C1"},{"value":"1,68E-04","module":"C2"},{"value":"0,0E+00","module":"C3"},{"value":"1,67E-05","module":"C4"},{"value":"-5,22E-04","module":"D"}]}],"end_of_life_flow":[{"parameter":"CRU","unit":"kg","values":[{"value":"0,0E+00","module":"A1-A3"},{"value":"0,0E+00","module":"A4"},{"value":"0,0E+00","module":"A5"},{"value":"0,0E+00","module":"C1"},{"value":"0,0E+00","module":"C2"},{"value":"0,0E+00","module":"C3"},{"value":"0,0E+00","module":"C4"},{"value":"0,0E+00","module":"D"}]},{"parameter":"MFR","unit":"kg","values":[{"value":"1,88E+01","module":"A1-A3"},{"value":"0,0E+00","module":"A4"},{"value":"0,0E+00","module":"A5"},{"value":"0,0E+00","module":"C1"},{"value":"0,0E+00","module":"C2"},{"value":"2,74E-01","module":"C3"},{"value":"0,0E+00","module":"C4"},{"value":"0,0E+00","module":"D"}]},{"parameter":"MER","unit":"kg","values":[{"value":"8,81E+00","module":"A1-A3"},{"value":"0,0E+00","module":"A4"},{"value":"0,0E+00","module":"A5"},{"value":"0,0E+00","module":"C1"},{"value":"0,0E+00","module":"C2"},{"value":"1,15E+02","module":"C3"},{"value":"0,0E+00","module":"C4"},{"value":"0,0E+00","module":"D"}]},{"parameter":"EEE","unit":"MJ","values":[{"value":"6,14E+00","module":"A1-A3"},{"value":"0,0E+00","module":"A4"},{"value":"0,0E+00","module":"A5"},{"value":"0,0E+00","module":"C1"},{"value":"0,0E+00","module":"C2"},{"value":"7,29E+01","module":"C3"},{"value":"0,0E+00","module":"C4"},{"value":"0,0E+00","module":"D"}]},{"parameter":"EET","unit":"MJ","values":[{"value":"9,29E+01","module":"A1-A3"},{"value":"0,0E+00","module":"A4"},{"value":"0,0E+00","module":"A5"},{"value":"0,0E+00","module":"C1"},{"value":"0,0E+00","module":"C2"},{"value":"1,10E+03","module":"C3"},{"value":"0,0E+00","module":"C4"},{"value":"0,0E+00","module":"D"}]}]}