ENVIRONMENTAL PRODUCT DECLARATION
as per ISO 14025 and EN 15804+A2
Owner of the Declaration Knauf Ceiling Solutions GmbH & Co. KG
Publisher Institut Bauen und Umwelt e.V. (IBU)
Programme holder Institut Bauen und Umwelt e.V. (IBU)
Declaration number EPD-KNA-20240276-IBA1-EN
Issue date 26/11/2024
Valid to 25/11/2029
ADAGIO dB+ and ADAGIO Acoustic+ Vector (24 mm)
Knauf Ceiling Solutions GmbH & Co. KG
www.ibu-epd.com | https://epd-online.com
1. General Information
Knauf Ceiling Solutions GmbH & Co. KG ADAGIO dB+ and ADAGIO Acoustic+ Vector (24
mm)
Programme holder Owner of the declaration
IBU – Institut Bauen und Umwelt e.V. Knauf Ceiling Solutions GmbH & Co. KG
Hegelplatz 1 Elsenthal 15
10117 Berlin 94481 Grafenau
Germany Germany
Declaration number Declared product / declared unit
EPD-KNA-20240276-IBA1-EN 1 m² ADAGIO dB+ and ADAGIO Acoustic+ (Vector) mineral ceiling tiles
with a surface weight of 8.66 kg/m².
This declaration is based on the product category rules: Scope:
Mineral panels, 01/08/2021 This document refers to 1 m² ADAGIO dB+ (all edges) and ADAGIO
(PCR checked and approved by the SVR) Acoustic+ (Vector edge) mineral ceiling tiles with a surface weight of
8.66 kg/m² and a thickness of 24 mm, manufactured at the production
facility in Grafenau, Germany.
Issue date
The owner of the declaration shall be liable for the underlying information
26/11/2024
and evidence; the IBU shall not be liable with respect to manufacturer
information, life cycle assessment data and evidences.
Valid to
The EPD was created according to the specifications of EN 15804+A2. In
25/11/2029 the following, the standard will be simplified as EN 15804.
Verification
The standard EN 15804 serves as the core PCR
Independent verification of the declaration and data according to ISO
14025:2011
internally X externally
Dipl.-Ing. Hans Peters
(Chairman of Institut Bauen und Umwelt e.V.)
Florian Pronold Dr.-Ing. Nikolay Minkov,
(Managing Director Institut Bauen und Umwelt e.V.) (Independent verifier)
1 Environmental Product Declaration - Knauf Ceiling Solutions GmbH & Co. KG - ADAGIO dB+ and ADAGIO Acoustic+ Vector (24 mm)
2. Product
In addition, dispersion paints are used on the surface and water
2.1 Product description/Product definition for preparation during production. The recycled content is
The ceiling tiles are manufactured using a wet-felt process and 36.8 %.
consist of biosoluble mineral wool, perlite, clay and starch. The
ceiling tiles meet the requirements of DIN 18177 and DIN EN This product/article/at least one partial article contains
13964. substances listed in the ECHA-candidate list (date: 25.06.2020)
exceeding 0.1 percentage by mass: No
The mineral tiles are available in a wide range of different
surface designs and product properties. Depending on the This product/article/at least one partial article contains other
design, the ceiling tiles are available in different formats and carcinogenic, mutagenic, reprotoxic (CMR) substances in
edge finishes. categories 1A or 1B which are not on the candidate list,
exceeding 0.1 percentage by mass: No
This EPD applies to the following products:
ADAGIO dB+ (all edges), ADAGIO Acoustic+ (Vector edge) Biocide products were added to this construction product or it
has been treated with biocide products (this then concerns a
For the placing on the market of the product in the European treated product as defined by the (EU) Ordinance on Biocide
Union/European Free Trade Association (EU/EFTA) (with the Products No. 528/2012): No
exception of Switzerland) Regulation (EU) No. 305/2011 (CPR)
applies. The product needs a declaration of performance taking In-can preservatives are used in the production process;
into consideration EN 13964:2014, suspended ceiling however, they are not part of the products and are therefore not
requirements and test methods and the CE-marking. For the within the scope of the Ordinance on Biocide Products.
application and use the respective national provisions apply.
2.6 Manufacture
2.2 Application The mineral tiles are produced in the traditional wet process
Mineral tiles (wet-felt) are typically used as lay in for suspended (wet-felt). The raw materials are mixed with water to form a
ceiling constructions. They are primarily used as optical homogeneous suspension, which is pumped onto a belt
cladding, but also for sound absorption and sound insulation, conveyor (Fourdrinier). The water is removed mechanically
for fire resistance and against fire spreading, for cleanrooms (gravity and vacuum) and by evaporation in the drying oven. As
and high hygiene requirements. far as possible, the process water is reused. It is treated
accordingly and fed back into the process water circuit.
2.3 Technical Data
Depending on the desired appearance the panels can be
Mineral boards (wet-felt) are regulated by EN 13964 and have sanded, colour-treated, patterned, eroded or embossed.
corresponding labelling and declaration of performance. The Production waste and dust are reused in the process in the
following data provide an overview of results: sense of an internal cycle.
Construction data (according to DIN 18177) The manufacturing plant is certified according to ISO 9001, ISO
14001, ISO 45001 and ISO 50001.
Name Value Unit
Thermal conductivity 0.075 W/(mK) 2.7 Environment and health during manufacturing
Sound absorption coefficient acc. ISO 354 and The manufacturer complies with the special German and
0.65(H) %
ISO 11654 European regulations for the production of mineral slabs:
Airborne sound reduction acc. ISO 10848 and
38 - 41 dB • The manufacturing plant is certified according to ISO
EN 717-1
9001, ISO 14001, ISO 45001 and ISO 50001.
Gross density 361 kg/m3 • The production has a closed water cycle.
• Production generates almost no waste, resulting blanks,
Performance data of the product in accordance with the
dust and rejects are reused.
declaration of
• Exclusive use of mineral fibres according to Regulation
performance with respect to its essential characteristics
(EU) No.1272/2008 Note Q.
according to EN 13964:2014, suspended ceiling requirements
• Prohibition of the production and use of biopersistent
and test methods (not part of CE-marking).
fibres (Ordinance on Hazardous Substances, Annex II,
2.4 Delivery status No. 5).
• Prohibition of placing biopersistent fibres on the market
The EPD refers to ADAGIO Acousitc+ dB (all edges) and
(Chemicals Prohibition Order, No.23 of the Annex to
ADAGIO Acoustic+ (Vector edge) 24 mm ceiling tiles which can
§1).
have variable length and width dimensions.
• Not subject to declaration according to REACH.
2.5 Base materials/Ancillary materials
2.8 Product processing/Installation
Mineral tile composition:
There are no recognised systemic hazards associated with the
Name Value Unit installation of ceiling tiles. It is recommended that materials are
Mineral wool 30 - 35 % handled in a manner that minimises dust generation. Workers
should wear appropriate personal protective equipment.
Perlite 5 - 10 %
Equipment such as gloves, goggles and dust masks are
Clay 30 - 35 %
recommended to minimise exposure to dust and prevent skin
Cellulose fibres 0 - 5 %
irritation.
Starch 5 - 10 %
2.9 Packaging
others 0 - 5 %
The panels are packaged with cardboard boxes and sealed
Brokes / Dust 25 - 30 %
with transparent polyethylene film. These packages lie on
2 Environmental Product Declaration - Knauf Ceiling Solutions GmbH & Co. KG - ADAGIO dB+ and ADAGIO Acoustic+ Vector (24 mm)
chemically untreated wooden pallets. The pallets are wrapped
Fire Reaction
with polyethylene stretch film. Foil, paper and wood can be
Name Value
recycled in the usual ways.
Building material class A2
2.10 Condition of use Smoke gas development s1
When handled properly, the mechanical and structural-physical
Burning droplets d0
properties of the mineral tile remain intact throughout its entire
service life. Direct contact with water should be avoided due to
the water-soluble binding agent starch. Water
In the case of prolonged contact with water, the starch binder
2.11 Environment and health during use dissolves, which can lead to a loss of structure, and if the
When properly installed, no dust/particles are released during soluble components are discharged into the sewage treatment
the use phase. For the substance groups formaldehyde, volatile plant, they are biodegradable, increasing the chemical oxygen
organic compounds (VOCs) and total volatile organic demand (COD) and the biological oxygen demand (BOD).
compounds (TVOCs), the limits according to DIN 18177 are
complied with. Mechanical destruction
The mineral slabs (wet-felt) can be broken by hand and also
2.12 Reference service life damaged superficially, which can result in minor dust formation.
The service life of the mineral tiles (wet-felted) is up to 50
years, depending on the area of use, exposure and state of 2.14 Re-use phase
maintenance. Within the framework of the conditions of use, no If the panels are removed properly, they can be reinstalled. In
ageing effects are to be expected apart from visual case of minor damage, the slabs can be reused as cut-to-size
discolouration caused by air circulation. tiles. Mineral tiles can be returned to the manufacturing process
if they are of the correct type and have sufficient material
2.13 Extraordinary effects quality; they can be recycled up to 100 %.
Fire
The declared products are classified in the fire reaction class 2.15 Disposal
A2-s1, d0 according to EN 13501-1. This means that they are The waste code number of production residues for mineral tiles
"non-combustible" according to the German building authority according to the AVV, German List of Wastes Ordinance is 10
designation (and also many other European countries) with 11 03, the waste code number for construction site waste
negligible smoke development and no burning drip in the event (offcuts) is 17 06 04. If the tiles are not recycled as described in
of fire. 2.14., they are disposed of in a landfill.
2.16 Further information
Further information at www.knaufceilingsolutions.com
3. LCA: Calculation rules
ceiling tiles are produced in the wet-felt process. Main raw
3.1 Declared Unit material inputs, therefore, refer to mineral wool, perlite, clay and
This EPD refers to a declared unit of 1 m² ADAGIO dB+ and starch. The production site is supplied with electricity from the
Adagio Acoustic+ mineral ceiling tiles with a surface weight of German power grid (considered based on the German residual
8.66 kg/m² and a thickness of 24 mm. mix) and thermal energy from natural gas. Also, the packaging
Declared Unit of the products is considered.
Name Value Unit
Module C1 | Deconstruction and demolition
Declared unit 1 m2 Disassembly of the product is done either manually or using
Grammage 8.66 kg/m2 smaller tools. Referring energy demand is considered to be
Layer thickness 0.024 m negligible.
The ceiling tiles are produced at the Knauf Ceiling Solutions
Modul C2 | Transport to disposal
production site in Grafenau, Germany.
The transport to the disposal of the material is estimated
declaring a 50 km radius to the landfill. In reality, this scenario
Both products share the identical recipe, coating, density and
may vary depending on the actual location of deconstruction
thickness. As only the edge detail differs, both products are
and referring waste treatment.
covered in one EPD.
Module C3 | Waste processing
As the declaration refers to specific products, no averages had
The declared scenario assumes landfilling of the product.
to be calculated.
Referring environmental impacts are accounted for in module
C4.
3.2 System boundary
The life cycle assessment of ADAGIO dB+ and ADAGIO
Module C4 | Disposal
Acoustic+ mineral ceiling tiles includes a cradle-to-gate analysis
Module C4 refers to the emissions from the disposal of the
of the products' environmental impacts with modules C1–C4
mineral ceiling tiles. The chosen scenario, therefore, includes
and module D (A1–A3, + C + D). Subsequent life cycle phases
the environmental burdens of landfilling of the product.
are part of the analysis:
Module D | Benefits and loads beyond the system
Module A1–A3 | Production stage
boundary
The production stage includes the upstream burdens of raw
The declared scenario assumes landfilling of the product.
material supply, their transports and the manufacturing plant of
Referring environmental impacts are accounted for in module
Knauf Ceiling Solutions located in Grafenau (Germany). Mineral
3 Environmental Product Declaration - Knauf Ceiling Solutions GmbH & Co. KG - ADAGIO dB+ and ADAGIO Acoustic+ Vector (24 mm)
C4. were used instead. The implemented MLC background
datasets refer to the latest versions available and are carefully
3.3 Estimates and assumptions chosen.
Assumptions and approximations are applied in case of a lack
of representative data. All assumptions and approximations are 3.7 Period under review
documented precisely and represent a best-guess Foreground data were collected in the 2023 production year,
representation of reality. In case of uncertainty, a conservative and the data are based on the volumes produced on an annual
approach is chosen. basis.
3.4 Cut-off criteria 3.8 Geographic Representativeness
The LCA model covers all available input and output flows, Land or region, in which the declared product system is
which can be represented based on robust data. Data gaps are manufactured, used or handled at the end of the product´s
filled with conservative assumptions from average data (when lifespan: Germany
available) or with generic data and are documented
accordingly. Only data with a contribution lower 1 % were cut
3.9 Allocation
off. Thus, no data were neglected, of which a substantial impact
is to be expected. All relevant data were collected All information for the allocation of given material and energy
comprehensively. Cut-off material and energy flows were flows is based on the ERP-systems of the production site.
chosen carefully based on their expected quantitative Annual input quantities are only available for the overall
contribution as well as potential environmental impacts. Thus, it production site. Thus, the calculation of specific input quantities
can be assumed that the sum of all neglected input flows does for the raw board production is based on their respective
not account for more than 5 % of the total material, water and recipe. In addition, product specific application rates of
energy flows. backcoat and primer were available. The total annual energy
consumption as well as waste quantities were broken down to
3.5 Background data the product under study based on their production share
This study uses generic background data for the evaluation of (produced square meters).
upstream environmental impacts from MLC 2023.2 database in
the LCA FE-software version 10. Knauf Ceiling Solutions uses waste paper and waste fibre glass
as secondary material. Waste paper reaches its end of waste
3.6 Data quality status after sorting of the paper, waste fibre glass after sorting
Data collection is based on product-specific questionnaires. It and grinding. As a result, the upstream supply chain of waste
follows an iterative process clarifying questions via e-mail, paper and waste fibre glass are considered burden-free. The
telephone calls or in personal/web meetings. Intensive system boundary for secondary raw materials defined in EN
discussions between Knauf Ceiling Solutions and Daxner & 15804 applies.
Merl result in an accurate mapping of product-related material
and energy flows. This leads to a high quality of foreground 3.10 Comparability
data collected. Data collection relies on a consistent process Basically, a comparison or an evaluation of EPD data is only
according to ISO 14044. possible if all the data sets to be compared were created
according to EN 15804 and the building context, respectively
The technological, geographical and time-related the product-specific characteristics of performance, are taken
representativeness of the database was kept in mind when into account.
selecting background data. Whenever specific data were The MLC 2023.2 background database (former GaBi) in the
missing, either generic datasets or representative average data LCA FE-software version 10 was used to calculate the LCA.
4. LCA: Scenarios and additional technical information
A3.
Characteristic product properties of biogenic carbon
Assembly (A5)
The biogenic carbon content quantifies the amount of biogenic
The End-of-Life of the product packaging is not declared in
carbon in the declared product.
module A5.
Information on the description of the biogenic carbon
Name Value Unit
content at the factory gate
Packaging (cardboard) 0.059 kg/m²
Name ValueUnit
Packaging (pallets) 0.166 kg/m²
kg
Biogenic carbon content in product 0.28 Packaging (polyethylene foil) 0.018 kg/m²
C
Biogenic carbon content in accompanying kg
0.1
packaging C End-of-Life (C1–4)
Note: 1 kg of biogenic carbon is equivalent to 44/12 kg of CO 2. Name Value Unit
Collected separately waste type 8.66 kg
Landfilling 8.66 kg
As the End-of-Life of the product packaging is not declared in
module A5, its carbon uptake is not considered in module A1–
4 Environmental Product Declaration - Knauf Ceiling Solutions GmbH & Co. KG - ADAGIO dB+ and ADAGIO Acoustic+ Vector (24 mm)
5. LCA: Results
The following table contains the LCA results for a declared unit of 1 m² ADAGIO dB+ and ADAGIO Acoustic+ mineral ceiling tiles with a
surface weight of 8.66 kg/m² and a thickness of 24 mm.
DESCRIPTION OF THE SYSTEM BOUNDARY (X = INCLUDED IN LCA; MND = MODULE OR INDICATOR NOT DECLARED; MNR
= MODULE NOT RELEVANT)
Benefits and
Construction loads beyond
Product stage Use stage End of life stage
process stage the system
boundaries
la ire ta m w a Ry lp p u s tro p s n a rT g n iru tc a fu n a M e h t m o rf tro p s n a rTe tis e h t o t e ta g y lb m e s s A e s U e c n a n e tn ia M ria p e R tn e m e c a lp e R tn e m h s ib ru fe R y g re n e la n o ita re p Oe s u re ta w la n o ita re p Oe s u n o itc u rts n o c -e Dn o itilo m e d tro p s n a rT g n is s e c o rp e ts a W la s o p s iD -e s u e R-y re v o c e R-g n ilc y c e Rla itn e to p
A1 A2 A3 A4 A5 B1 B2 B3 B4 B5 B6 B7 C1 C2 C3 C4 D
X X X MND MND MND MND MNR MNR MNR MND MND X X X X X
RESULTS OF THE LCA - ENVIRONMENTAL IMPACT according to EN 15804+A2: 1 m² ADAGIO dB+, ADAGIO Acoustic+ mineral
ceiling tiles (8.66 kg/m²)
Parameter Unit A1-A3 C1 C2 C3 C4 D
Global Warming Potential total (GWP-total) kg CO 2 eq 4.93E+00 0 3.16E-02 0 1.17E+00 0
Global Warming Potential fossil fuels (GWP-fossil) kg CO 2 eq 6.32E+00 0 3.12E-02 0 1.28E-01 0
Global Warming Potential biogenic (GWP-biogenic) kg CO 2 eq -1.4E+00 0 7.14E-05 0 1.04E+00 0
Global Warming Potential luluc (GWP-luluc) kg CO 2 eq 3.54E-03 0 2.92E-04 0 4.04E-04 0
Depletion potential of the stratospheric ozone layer (ODP) kg CFC11 eq 5.46E-10 0 4.11E-15 0 3.31E-13 0
Acidification potential of land and water (AP) mol H+ eq 2.95E-02 0 1.12E-04 0 9.23E-04 0
Eutrophication potential aquatic freshwater (EP-freshwater) kg P eq 1.66E-04 0 1.15E-07 0 2.62E-07 0
Eutrophication potential aquatic marine (EP-marine) kg N eq 6.15E-03 0 5.13E-05 0 2.39E-04 0
Eutrophication potential terrestrial (EP-terrestrial) mol N eq 9.51E-02 0 5.76E-04 0 2.62E-03 0
Formation potential of tropospheric ozone photochemical oxidants kg NMVOC
1.11E-02 0 1.01E-04 0 7.2E-04 0
(POCP) eq
Abiotic depletion potential for non fossil resources (ADPE) kg Sb eq 1.11E-06 0 2.09E-09 0 6.01E-09 0
Abiotic depletion potential for fossil resources (ADPF) MJ 9.57E+01 0 4.3E-01 0 1.73E+00 0
m3 world eq
Water use (WDP) 3.29E+00 0 3.81E-04 0 1.43E-02 0
deprived
RESULTS OF THE LCA - INDICATORS TO DESCRIBE RESOURCE USE according to EN 15804+A2: 1 m² ADAGIO dB+, ADAGIO
Acoustic+ mineral ceiling tiles (8.66 kg/m²)
Parameter Unit A1-A3 C1 C2 C3 C4 D
Renewable primary energy as energy carrier (PERE) MJ 9.28E-01 0 3.13E-02 0 2.82E-01 0
Renewable primary energy resources as material utilization
MJ 1.6E+01 0 0 0 0 0
(PERM)
Total use of renewable primary energy resources (PERT) MJ 1.7E+01 0 3.13E-02 0 2.82E-01 0
Non renewable primary energy as energy carrier (PENRE) MJ 9.57E+01 0 4.32E-01 0 1.73E+00 0
Non renewable primary energy as material utilization (PENRM) MJ 0 0 0 0 0 0
Total use of non renewable primary energy resources (PENRT) MJ 9.57E+01 0 4.32E-01 0 1.73E+00 0
Use of secondary material (SM) kg 9.57E-01 0 0 0 0 0
Use of renewable secondary fuels (RSF) MJ 0 0 0 0 0 0
Use of non renewable secondary fuels (NRSF) MJ 0 0 0 0 0 0
Use of net fresh water (FW) m3 2.6E+00 0 3.43E-05 0 4.38E-04 0
RESULTS OF THE LCA – WASTE CATEGORIES AND OUTPUT FLOWS according to EN 15804+A2:
1 m² ADAGIO dB+, ADAGIO Acoustic+ mineral ceiling tiles (8.66 kg/m²)
Parameter Unit A1-A3 C1 C2 C3 C4 D
Hazardous waste disposed (HWD) kg 1.93E-05 0 1.34E-12 0 3.78E-11 0
Non hazardous waste disposed (NHWD) kg 9.98E-01 0 6.58E-05 0 8.67E+00 0
Radioactive waste disposed (RWD) kg 2.42E-03 0 8.08E-07 0 1.97E-05 0
Components for re-use (CRU) kg 0 0 0 0 0 0
Materials for recycling (MFR) kg 0 0 0 0 0 0
Materials for energy recovery (MER) kg 0 0 0 0 0 0
Exported electrical energy (EEE) MJ 0 0 0 0 0 0
Exported thermal energy (EET) MJ 0 0 0 0 0 0
RESULTS OF THE LCA – additional impact categories according to EN 15804+A2-optional:
1 m² ADAGIO dB+, ADAGIO Acoustic+ mineral ceiling tiles (8.66 kg/m²)
Parameter Unit A1-A3 C1 C2 C3 C4 D
5 Environmental Product Declaration - Knauf Ceiling Solutions GmbH & Co. KG - ADAGIO dB+ and ADAGIO Acoustic+ Vector (24 mm)
Disease
Incidence of disease due to PM emissions (PM) 2.57E-07 0 6.7E-10 0 1.14E-08 0
incidence
Human exposure efficiency relative to U235 (IR) kBq U235 eq 3.05E-01 0 1.2E-04 0 2.28E-03 0
Comparative toxic unit for ecosystems (ETP-fw) CTUe 2E+01 0 3.08E-01 0 9.37E-01 0
Comparative toxic unit for humans (carcinogenic) (HTP-c) CTUh 4.49E-09 0 6.25E-12 0 1.46E-10 0
Comparative toxic unit for humans (noncarcinogenic) (HTP-nc) CTUh 8.76E-08 0 2.78E-10 0 1.54E-08 0
Soil quality index (SQP) SQP 7.65E+01 0 1.8E-01 0 4.21E-01 0
Disclaimer 1 – for the indicator 'Potential Human exposure efficiency relative to U235'.
This impact category deals mainly with the eventual impact of low-dose ionizing radiation on human health of the nuclear fuel cycle. It
does not consider effects due to possible nuclear accidents, occupational exposure or radioactive waste disposal in underground
facilities. Potential ionizing radiation from the soil, radon and from some construction materials is also not measured by this indicator.
Disclaimer 2 – for the indicators 'abiotic depletion potential for non-fossil resources', 'abiotic depletion potential for fossil resources',
'water (user) deprivation potential, deprivation-weighted water consumption', 'potential comparative toxic unit for ecosystems', 'potential
comparative toxic unit for humans – cancerogenic', 'Potential comparative toxic unit for humans - not cancerogenic', 'potential soil
quality index'. The results of this environmental impact indicator shall be used with care as the uncertainties on these results are high
as there is limited experience with the indicator.
6. LCA: Interpretation
The following interpretation contains a summary of the LCA
results referenced to a declared unit of 1 m² ADAGIO dB+ and
ADAGIO Acoustic+ mineral ceiling tiles.
The comparison of the product's life cycle phases shows a C4) have a minor contribution.
clear dominance of the production phase (modules A1–A3) in
all environmental impact categories. The potential The upstream supply chain of the raw board plays a dominant
environmental impacts from transport to disposal (module C2) role in the carbon footprint.
and the End-of-Life of the products due to landfilling (module
7. Requisite evidence
Testing Date: 23.06.2021
7.1 Radioactivity
Measurements of radioactivity did not reveal any evidence of 7.2 Biopersistence
artificial radioactivity outside the natural background radiation. The mineral wool used for the production of the panels is
Measuring point: TÜV Süd Industrie Service biosoluble and, according to EU Regulation 1272/2008/EC, is
to be assessed as free of suspected cancer. The "RAL Mineral
Test Number: G 7299 002 Wool Quality Seal" monitors and guarantees the quality of the
6 Environmental Product Declaration - Knauf Ceiling Solutions GmbH & Co. KG - ADAGIO dB+ and ADAGIO Acoustic+ Vector (24 mm)
wool used. Test basis: ISO 16000-6
The production and use of non-exempt fibres is prohibited by
AgBB Overview (28 days)
the Ordinance on Hazardous Substances and the Chemicals
Name Value Unit
Prohibition Ordinance.
TVOC (C6 - C16) 44 μg/m3
7.3 VOC emissions Sum SVOC (C16 - C22) < 5 μg/m3
Measuring point: Eurofins Product Testing A/S
R (dimensionless) 0,031
Test report: VOC emission test report Indoor Air Comfort GOLD
VOC without NIK < 5 μg/m3
(10.11.2022)
Number: 392-2022-00121902_A_EN Carcinogenic substances < 1 μg/m3
Testing periode: 05.10.2022 - 10.11.2022
8. References
Standards
DIN 18177 ISO 16000-6
DIN 18177:2012, Mineral tiles manufactured in the factory by ISO 16000-6:2011-12, Indoor air contaminants - Part 6:
the wet felt process - Characteristic values and test methods. Determination of VOCs in indoor air and test chambers,
sampling on Tenax TA®, thermal desorption and gas
EN 13501-1 chromatography with MS/FID.
DIN EN 13501-1:2019, Classification of construction products
and building elements according to their reaction to fire, Part 1: ISO 45001
Classification with the results of tests on the reaction to fire of DIN ISO 45001:2018-06, Occupational health and safety
construction products. management systems - Requirements with guidance for use.
EN 13964 ISO 50001
DIN EN 13964:2014, Suspended ceilings - Requirements and DIN EN ISO 50001:2011-12, Energy management systems -
test methods. Requirements with guidance for use.
EN 15804
DIN EN 15804:2012+A2:2019, Sustainability of construction Further References
works - Environmental product declarations - Core rules for the
product category of construction products. AgBB
Ausschuss zur gesundheitlichen Bewertung von Bauprodukte
ISO 354 (AgBB) (Committee for health-related evaluation of building
DIN EN ISO 354:2003-12, Acoustics - Measurement of sound products): Vorgehensweise bei der gesundheitlichen
absorption in reverberant rooms. Bewertung der Emissionen von flüchtigen organischen
Verbindungen (VOC und SVOC) aus Bauprodukten.
ISO 717-1
DIN EN ISO 717-1:2013-06, Acoustics - Assessment of sound AVV, German List of Wastes Ordinance
insulation in buildings and of building elements - Part 1: Regulation on the European Waste List.
Airborne sound insulation.
Chemicals Prohibition Ordinance
ISO 9001 Chemicals Prohibition Ordinance (German designation:
DIN EN ISO 9001:2015-11,Quality management systems - Chemikalien-Verbotsverordnung – ChemVerbotsV) of 20
Requirements. January 2017 (Federal Law Gazette I p. 94; 2018 I p. 1389),
last amended by Article 300 of the Ordinance of 19 June 2020
ISO 10848-2 (Federal Law Gazette I p. 1328).
DIN EN ISO 10848-2:2006-08, Acoustics - Measurement of
airborne and impact sound transmission between adjacent ECHA-candidate list
rooms in test stands - Part 2: Application to lightweight List of substances of very high concern (SVHC) for
components where the connection has a minor influence. authorisation (ECHA Candidate List), 25.06.2020, published
under Article 59(10) of REACH. Helsinki: European Chemicals
ISO 11654 Agency.
DIN EN ISO 11654:1997-07, Acoustics - Sound absorbers for
use in buildings - Evaluation of sound absorption. Eurofins Product Testing A/S
Test report: VOC emission test report Indoor Air Comfort GOLD
ISO 14001 (10.11.2022), Number: 392-2022-00121902_A_EN.
DIN EN ISO 14001:2015-11, Environmental management
systems - Requirements with guidance for use. IBU 2021
General instructions for the EPD program of Institut Bauen und
ISO 14025 Umwelt e.V. (IBU). Version 2.0, Berlin: Institut Bauen und
DIN EN ISO 14025:2011-10, Environmental labels and Umwelt e.V., 2021. www.ibu-epd.com
declarations — Type III environmental declarations —
Principles and procedures. LCA FE
LCA FE 10, LCA for Experts Software System and Database for
ISO 14044 Life Cycle Engineering. Version 10.7.1.28. Sphera, 1992-2023.
DIN EN ISO 14044:2006-10, Environmental management – Life
cycle assessment – Requirements and guidelines.
7 Environmental Product Declaration - Knauf Ceiling Solutions GmbH & Co. KG - ADAGIO dB+ and ADAGIO Acoustic+ Vector (24 mm)
MLC including plants and fibre types, as of January 2021.
MLC 2023.2, Database for Life Cycle Engineering implemented
in LCA for Experts software system. DB v10.7 2023.2. Sphera, REACH
1992-2023. Available at: Regulation (EC) No 1907/2006 of the European Parliament and
https://sphera.com/productsustainabilitygabidatasearch/. Council from 18 December 2006, Regulation concerning the
Registration, Evaluation, Authorisation and Restriction of
Ordinance on Biocide Products Chemicals (REACH).
Regulation (EU) No 528/2012 of the European Parliament and
of the Council of 22 May 2012 concerning the making available Regulation (EU) Nr. 305/2011(CPR)
on the market and use of biocidal products. Regulation (EU) No 305/2011 of the European Parliament and
of the Council of 9 March 2011 laying down harmonised
Ordinance on Hazardous Substances conditions for the marketing of construction products and
Ordinance on Hazardous Substances, of 26 November 2010 repealing Council Directive 89/106/EEC Text with EEA
(Federal Law Gazette I p. 1643, 1644), last amended by Article relevance.
148 of the Law of 29 March 2017 (Federal Law Gazette I p.
626). Regulation (EU) Nr.1272/2008
Regulation (EC) No 1272/2008 of the European Parliament and
PCR Part A of the Council of 16 December 2008 on classification, labelling
Product category rules for buildingrelated products and and packaging of substances and mixtures, amending and
services. Part A: Calculation rules for the life cycle assessment repealing Directives 67/548/EEC and 1999/45/EC, and
and requirements for the project report in accordance with EN amending Regulation (EC) No 1907/2006.
15804+A2:2019. Version 1.3. Berlin: Institut Bauen und Umwelt
e.V. (eds.), 2022. TÜV Süd Industrie Service
TÜV Strahlenmesslabor. IS-ETS1-MUC/er.
PCR: Mineral panels
Institut Bauen und Umwelt e.V. (IBU), 2023. Product Category
Rules for Building-Related Products and Services. Part B:
Requirements on the EPD for Mineral panels. Version 8.
19.10.2023.
RAL Mineral Wool Quality Seal
GGM members with the right to use the RAL quality mark
8 Environmental Product Declaration - Knauf Ceiling Solutions GmbH & Co. KG - ADAGIO dB+ and ADAGIO Acoustic+ Vector (24 mm)
Publisher
Institut Bauen und Umwelt e.V. +49 (0)30 3087748- 0
Hegelplatz 1 info@ibu-epd.com
10117 Berlin www.ibu-epd.com
Germany
Programme holder
Institut Bauen und Umwelt e.V. +49 (0)30 3087748- 0
Hegelplatz 1 info@ibu-epd.com
10117 Berlin www.ibu-epd.com
Germany
Author of the Life Cycle Assessment
Daxner & Merl GmbH +43 676 849477826
Schleifmühlgasse 13/24 office@daxner-merl.com
1040 Wien www.daxner-merl.com
Austria
Owner of the Declaration
Knauf Ceiling Solutions GmbH & Co. KG 0049 8552 422 0
Elsenthal 15 ceiling.solutions@knauf.com
94481 Grafenau www.knaufceilingsolutions.com
Germany
9 Environmental Product Declaration - Knauf Ceiling Solutions GmbH & Co. KG - ADAGIO dB+ and ADAGIO Acoustic+ Vector (24 mm)
