ENVIRONMENTAL PRODUCT DECLARATION
as per ISO 14025 and EN 15804+A2
Owner of the Declaration dormakaba International Holding GmbH
Publisher Institut Bauen und Umwelt e.V. (IBU)
Programme holder Institut Bauen und Umwelt e.V. (IBU)
Declaration number EPD-DOR-20220259-CBA1-EN
Issue date 29.11.2022
Valid to 28.11.2027
AL 401 Series Sliding Door Operator
Dormakaba
www.ibu-epd.com | https://epd-online.com
General Information
Dormakaba AL 401 Series Sliding Door Operator
Programme holder Owner of the declaration
IBU – Institut Bauen und Umwelt e.V. dormakaba International Holding GmbH
Hegelplatz 1 DORMA Platz 1
10117 Berlin 58256 Ennepetal
Germany Germany
Declaration number Declared product / declared unit
EPD-DOR-20220259-CBA1-EN 1 piece of the product: AL 401 Series - sliding door operator, consisting of
the following items:
- AL 401 profiles
- AL 401 drive components, consisting of motor, controller, power supply
- AL 401 belt drive components
- AL 401 accessories battery pack and lock - AL 401 carrier components -
additional mechanical components
- packaging
This declaration is based on the product category rules: Scope:
Drive systems for automatic doors and gates, 01.08.2021 The EPD refers to a specific automatic sliding door operator AL 401
(PCR checked and approved by the SVR) produced by dormakaba. The product site is located in Hallam, Australia.
The year of data collection is 2022.
Issue date The owner of the declaration shall be liable for the underlying information
and evidence; the IBU shall not be liable with respect to manufacturer
29.11.2022
information, life cycle assessment data and evidences.
The EPD was created according to the specifications of EN 15804+A2. In
Valid to
the following, the standard will be simplified as EN 15804.
28.11.2027
Verification
The standard EN 15804 serves as the core PCR
Independent verification of the declaration and data according to ISO
14025:2011
internally X externally
Dipl.-Ing. Hans Peters
(Chairman of Institut Bauen und Umwelt e.V.)
Florian Pronold Dr.-Ing. Wolfram Trinius,
(Managing Director Institut Bauen und Umwelt e.V.) (Independent verifier)
1 Environmental Product Declaration - Dormakaba - AL 401 Series Sliding Door Operator
Product
Product not harmonised in accordance with the CPR but in
Product description/Product definition accordance with:
The AL 401 is a heavy duty automatic door operator. Its unique
• Australian Standard AS5007
rubber-mounted stainless steel tracking system and heavy-duty
Delivery status:
cowl provide the product longevity, a load capacity of 400 kg
The declared AL 401 series sliding door operator includes the
maximum and installation alternatives.
profiles, drive, belt drive, carrier, battery pack and lock,
The AL 401 is designed to control and operate bi-parting and
mechanical components and packaging with a weight of 123,20
single sliding doors including aluminium framed and frameless
kg.
glass doors up to 19 mm thick.
Features
• High Security Locking
• Heavy Duty & Robust
• Purpose Designed Motor
• Fully Integrated UPS system
• State-of-the-Art Electronics
Base materials/Ancillary materials
For the placing on the market following legal provisions apply:
The AL 401 automatic sliding door operator comprises the
• Australian Standard AS 5007
following components including packaging:
• Endurance testing clause 4.4.1.1. and 4.4.2 by NATA
accredited facility
• 2011/65/EU ROHS3 Directive
Application
The dormakaba AL 401 automatic door operator is a proven
performer in airports, shopping centres, supermarkets, hotels,
hospitals, financial institutions, sports stadiums and many other
commercial sites.
The following parameters are applicable for single and double-
leaf doors:
Single-panel sliding door
• Maximum door width: 3000 mm
• Maximum door weight: 400 kg The product contains partial articles which contain substances
Double leaf sliding door listed in the Candidate List of REACH
Regulation 1907/2006/EC (date: 10.06.2022) exceeding 0.1
• Maximum door width: 2000 mm
percentage by mass: yes
• Maximum door weight: 200 kg
• Lead (Pb): 7439-92-1 (CAS-No) is used in the brass
Technical Data alloy. The concentration of lead in the alloy does not
The technical data of the AL 401 series are as follows: exceed 4 % (by mass).
Name Value Unit • The drive system is battery-powered (lead accumulator).
Height 240 mm
Reference service life
Installation depth 152 mm
The life cycle of the AL 401 series is about 10 years, depending
Opening speed maximum 50 cm/s on the application and frequency of use. Regular maintenance
Closing speed maximum 40 cm/s is advised to ensure the life expectancy of 10 years. For repairs
Hold open time maximum 60 s or renewals, suitable spare parts are available. The AL 401 is
tested and certified to 1,000,000 cycles according to AS 5007
Supply voltage, frequency maximum 60 Hz
NATA accredited.
Power consumption 175 W
Class of protection 20 IP
LCA: Calculation rules
Declared Unit Production - Module A1-A3
The declared unit is 1 piece of the product: AL 401 Series The product stage includes:
Sliding Door Operator — A1, raw material extraction, processing and mechanical
Declared unit treatments, processing of secondary material input (e.g.
recycling processes), — A2, transport to the manufacturer,
Name Value Unit
— A3, manufacturing and assembly including provision of all
Declared unit 1 pce.
materials, products and energy, as well as waste processing up
Mass (total system) (excl. packaging) 123,20 kg to the end-of waste state.
System boundary Construction stage - Modules A4-A5
The type of EPD is: cradle-to-gate with options, modules C1– The construction process stage includes:
C4, and module D (A1–A3 + C + D and additional modules: A4 — A4, transport to the building site;
+ A5 + B6) — A5, installation into the building;
2 Environmental Product Declaration - Dormakaba - AL 401 Series Sliding Door Operator
including provision of all materials, products and energy, as well Module D (Benefits and loads beyond the system boundary)
as waste processing up to the end-of-waste state or disposal of includes:
final residues during the construction process stage. — D, recycling potentials, expressed as net impacts and
benefits.
Use stage - Module B6
The use stage related to the operation of the building includes: Geographic Representativeness
— B6, operational energy use Land or region, in which the declared product system is
manufactured, used or handled at the end of the product´s
End-of-life stage– Modules C1-C4 and D lifespan: Australia
The end-of-life stage includes:
— C1, de-construction, demolition:
Comparability
— C2, transport to waste processing;
Basically, a comparison or an evaluation of EPD data is only
— C3, waste processing for reuse, recovery and/or recycling;
possible if all the data sets to be compared were created
— C4, disposal;
according to EN 15804 and the building context, respectively
including provision and all transport, provision of all materials,
the product-specific characteristics of performance, are taken
products and related energy and water use.
into account. Background database: GaBi, SP40.
LCA: Scenarios and additional technical information
Characteristic product properties of biogenic carbon
Information on describing the Biogenic Carbon Content at Operational energy use (B6)
factory gate The use stage is declared for 10 years
Name ValueUnit Name Value Unit
Biogenic carbon content in product 0.11 kg Electricity consumption for 1 year 93.84 kWh
C
Days per year in use 365 days
Biogenic carbon content in accompanying kg
0.52 On mode per day 1 h
packaging C
Idle mode per day 7 h
Note: 1 kg of biogenic carbon is equivalent to 44/12 kg of CO .
2 Off mode per day 16 h
On mode power 67,2 W
Idle mode power 7,7 W
The following technical scenario information is required for the
declared modules Off mode power 8,5 W
Transport from the gate to the site (A4) End of life (C1-C4)
Name Value Unit Name Value Unit
Litres of fuel (per 1 kg) 0.00276 l/100km Recycling 103 kg
Capacity utilisation (including empty runs) 55 % Energy recovery 3.4 kg
Transport distance via medium truck 100 km Landfilling 15.2 kg
Transport distance is declared for a distance of 100 km by truck Transport to waste management 50 km
in order to allow scaling to a specific point of installation.
The product is disassembled in a recycling process.
Material recycling is then assumed for the metals, electronics
Installation into the building (A5) and electromechanics. The plastic components are assumed to
Name Value Unit be incinerated with energy recovery. Minor proportions of
residues arising from the recycling process are landfilled.
Waste packaging (paper and plastic) 1.42 kg
Region for the End of Life is: Global.
Reference service life
Reuse, recovery and/or recycling potentials (D),
Name Value Unit
relevant scenario information
Life Span according to the manufacturer 10 a
The collection rate is 100 %.
3 Environmental Product Declaration - Dormakaba - AL 401 Series Sliding Door Operator
LCA: Results
DESCRIPTION OF THE SYSTEM BOUNDARY (X = INCLUDED IN LCA; MND = MODULE OR INDICATOR NOT DECLARED; MNR
= MODULE NOT RELEVANT)
Benefits and
Construction loads beyond
Product stage Use stage End of life stage
process stage the system
boundaries
la ire ta m w a Ry lp p u s tro p s n a rT g n iru tc a fu n a M e h t m o rf tro p s n a rTe tis e h t o t e ta g y lb m e s s A e s U e c n a n e tn ia M ria p e R tn e m e c a lp e R tn e m h s ib ru fe R y g re n e la n o ita re p Oe s u re ta w la n o ita re p Oe s u n o itc u rts n o c -e Dn o itilo m e d tro p s n a rT g n is s e c o rp e ts a W la s o p s iD -e s u e R-y re v o c e R-g n ilc y c e Rla itn e to p
A1 A2 A3 A4 A5 B1 B2 B3 B4 B5 B6 B7 C1 C2 C3 C4 D
X X X X X MND MND MNR MNR MNR X MND X X X X X
RESULTS OF THE LCA - ENVIRONMENTAL IMPACT according to EN 15804+A2: 1 piece AL 401 sliding door operator
Parameter Unit A1-A3 A4 A5 B6 C1 C2 C3 C4 D
GWP-total kg CO 2 eq 7.97E+02 1.08E+00 2.02E+00 9.42E+02 0 5.29E-01 9.4E+00 1.32E-01 -4.76E+02
GWP-fossil kg CO 2 eq 7.99E+02 1.03E+00 6.3E-02 9.41E+02 0 5.06E-01 8.66E+00 1.31E-01 -4.75E+02
GWP-biogenic kg CO 2 eq -2.67E+00 4.8E-02 1.96E+00 8.46E-01 0 2.3E-02 7.42E-01 4.49E-04 -1.09E+00
GWP-luluc kg CO 2 eq 5.91E-01 2.45E-05 3.38E-05 2.25E-01 0 1.2E-05 4.93E-04 3.78E-04 -1.49E-01
ODP kg CFC11 eq 4.96E-10 1.09E-16 3.68E-16 4.3E-12 0 5.34E-17 4.41E-15 4.87E-16 -3.2E-09
AP mol H+ eq 3.86E+00 1E-03 5.65E-04 4.52E+00 0 5.06E-04 2E-03 9.42E-04 -1.91E+00
EP-freshwater kg P eq 8.48E-04 2.2E-07 7.18E-08 4.38E-04 0 1.08E-07 7.03E-07 2.26E-07 -2.57E-04
EP-marine kg N eq 5.19E-01 3.28E-04 2.04E-04 9.67E-01 0 1.61E-04 3.62E-04 2.43E-04 -2.44E-01
EP-terrestrial mol N eq 5.65E+00 4E-03 3E-03 1.06E+01 0 2E-03 7E-03 3E-03 -2.64E+00
kg NMVOC
POCP 1.62E+00 9.27E-04 5.4E-04 2.69E+00 0 4.55E-04 1E-03 7.34E-04 -7.83E-01
eq
ADPE kg Sb eq 2E-02 3.09E-08 5.8E-09 6.31E-05 0 1.52E-08 6.06E-08 1.18E-08 -1E-02
ADPF MJ 1.02E+04 1.46E+01 6.4E-01 1.04E+04 0 7.17E+00 4.1E+00 1.72E+00 -6.53E+03
m3 world eq
WDP 1.3E+02 2E-03 2.5E-01 3.57E+02 0 9.91E-04 9.5E-01 1.4E-02 -3.95E+01
deprived
GWP = Global warming potential; ODP = Depletion potential of the stratospheric ozone layer; AP = Acidification potential of land and water; EP =
Eutrophication potential; POCP = Formation potential of tropospheric ozone photochemical oxidants; ADPE = Abiotic depletion potential for non-fossil
resources; ADPF = Abiotic depletion potential for fossil resources; WDP = Water (user) deprivation potential)
RESULTS OF THE LCA - INDICATORS TO DESCRIBE RESOURCE USE according to EN 15804+A2: 1 piece AL 401 sliding door
operator
Parameter Unit A1-A3 A4 A5 B6 C1 C2 C3 C4 D
PERE MJ 3.73E+03 4.6E-02 1.71E+01 1.59E+03 0 2.3E-02 1.15E+01 2.26E-01 -2.82E+03
PERM MJ 2.74E+01 0 -1.7E+01 0 0 0 -1.04E+01 0 0
PERT MJ 3.75E+03 4.6E-02 1.17E-01 1.59E+03 0 2.3E-02 1.06E+00 2.26E-01 -2.82E+03
PENRE MJ 1.01E+04 1.46E+01 8.55E-01 1.04E+04 0 7.18E+00 1.27E+02 1.72E+00 -6.53E+03
PENRM MJ 1.23E+02 0 -2.15E-01 0 0 0 -1.23E+02 0 0
PENRT MJ 1.02E+04 1.46E+01 6.4E-01 1.04E+04 0 7.18E+00 4.1E+00 1.72E+00 -6.53E+03
SM kg 1.28E+01 0 0 0 0 0 0 0 0
RSF MJ 0 0 0 0 0 0 0 0 0
NRSF MJ 0 0 0 0 0 0 0 0 0
FW m3 9.71E+00 8.26E-05 6E-03 5.01E+00 0 4.06E-05 2.3E-02 4.35E-04 -5.57E+00
PERE = Use of renewable primary energy excluding renewable primary energy resources used as raw materials; PERM = Use of renewable primary
energy resources used as raw materials; PERT = Total use of renewable primary energy resources; PENRE = Use of non-renewable primary energy
excluding non-renewable primary energy resources used as raw materials; PENRM = Use of non-renewable primary energy resources used as raw
materials; PENRT = Total use of non-renewable primary energy resources; SM = Use of secondary material; RSF = Use of renewable secondary fuels;
NRSF = Use of non-renewable secondary fuels; FW = Use of net fresh water
RESULTS OF THE LCA – WASTE CATEGORIES AND OUTPUT FLOWS according to EN 15804+A2:
1 piece AL 401 sliding door operator
Parameter Unit A1-A3 A4 A5 B6 C1 C2 C3 C4 D
HWD kg 1.55E-05 1.42E-09 9.57E-10 1.69E-06 0 6.96E-10 1.54E-08 2.63E-08 -4.5E-05
NHWD kg 1.75E+02 1E-03 6.4E-02 2.69E+00 0 7.34E-04 9.01E-01 8.67E+00 -1.09E+02
RWD kg 5.27E-01 1.57E-05 3.35E-05 2E-03 0 7.7E-06 1.54E-04 1.96E-05 -6.49E-01
CRU kg 0 0 0 0 0 0 0 0 0
MFR kg 0 0 0 0 0 0 1.09E+02 0 0
MER kg 0 0 0 0 0 0 0 0 0
EEE MJ 0 0 3.06E+00 0 0 0 0 0 0
EET MJ 0 0 5.56E+00 0 0 0 0 0 0
4 Environmental Product Declaration - Dormakaba - AL 401 Series Sliding Door Operator
HWD = Hazardous waste disposed; NHWD = Non-hazardous waste disposed; RWD = Radioactive waste disposed; CRU = Components for re-use;
MFR = Materials for recycling; MER = Materials for energy recovery; EEE = Exported electrical energy; EET = Exported thermal energy
RESULTS OF THE LCA – additional impact categories according to EN 15804+A2-optional:
1 piece AL 401 sliding door operator
Parameter Unit A1-A3 A4 A5 B6 C1 C2 C3 C4 D
Disease
PM 4.23E-05 5.42E-09 3.14E-09 4.6E-05 0 2.66E-09 2.01E-08 1.17E-08 -3.04E-05
incidence
IR kBq U235 eq 1.02E+02 2E-03 5E-03 2.53E-01 0 1E-03 1.4E-02 2E-03 -1.3E+02
ETP-fw CTUe 3.65E+03 1.04E+01 3.03E-01 1.43E+03 0 5.08E+00 1.55E+00 9.84E-01 -2.44E+03
HTP-c CTUh 1.49E-05 1.95E-10 1.61E-11 8.4E-08 0 9.56E-11 1.35E-10 1.46E-10 -1.86E-07
HTP-nc CTUh 1.08E-05 8.33E-09 7.09E-10 3.09E-06 0 4.09E-09 1.33E-08 1.61E-08 -3.35E-06
SQP SQP 1.37E+03 3.8E-02 1.7E-01 9.75E+02 0 1.8E-02 1.23E+00 3.59E-01 -2.47E+02
PM = Potential incidence of disease due to PM emissions; IR = Potential Human exposure efficiency relative to U235; ETP-fw = Potential comparative
Toxic Unit for ecosystems; HTP-c = Potential comparative Toxic Unit for humans (cancerogenic); HTP-nc = Potential comparative Toxic Unit for humans
(not cancerogenic); SQP = Potential soil quality index
Disclaimer 1 – for the indicator IRP
This impact category deals mainly with the eventual impact of low dose ionizing radiation on human health of the nuclear fuel cycle. It
does not consider effects due to possible nuclear accidents, occupational exposure nor radioactive waste disposal in underground
facilities.Potential ionizing radiation from the soil, from radon and from some construction materials is also not measured by this
indicator.
Disclaimer 2 – for the indicators ADPE, ADPF, WDP, ETP-fw, HTP-c, HTP-nc, SQP
The results of this environmental impact indicator shall be used with care as the uncertainties on these results are high or as there is
limited experience with the indicator.
References
Standards GaBi ts documentation
GaBi life cycle inventory data documentation
AS 5007 (https://www.gabisoftware.
AS 5007 -2007 com/support/gabi/gabidatabase- 2020-lci-documentation/).
Powered doors for pedestrian access and egress.
LCA-tool dormakaba
Further References LCA tool, ENS (drive system) LCA tool No.: IBU-DOR-202108-
LT1-EN Developed by Sphera Solutions GmbH.
2011/65/EU ROHS3 Directive
Directive 2011/65/EU of the European Parliament and of the PCR Part A
Council of 8 June 2011 on the restriction of the use of certain PCR – Part A: Calculation Rules for the Life Cycle Assessment
hazardous substances in electrical and electronic equipment. and Requirements on the Project Re-port according to EN
15804+A2:2019, Version 1.0, Institut Bauen und Umwelt e.V.,
IBU 2021 www.ibu-epd.com.
General Instructions for the EPD programme of Institut Bauen
und Umwelt e.V. PCR Part B
Version 2.0, Berlin: Institut Bauen und Umwelt e.V., 2021. PCR – Part B: Requirements on the EPD for Building Hardware
www.ibu-epd.com product, version 1.2, Institut Bauen und Umwelt e.V., www.ibu-
epd.com, 2020.
GaBi ts software
Sphera Solutions GmbH Gabi Software System and Database
for Life Cycle Engineering 1992-2020 Version 10.0.0.71
University of Stuttgart Leinfelden-Echterdingen
5 Environmental Product Declaration - Dormakaba - AL 401 Series Sliding Door Operator
Publisher
Institut Bauen und Umwelt e.V. +49 (0)30 3087748- 0
Hegelplatz 1 info@ibu-epd.com
10117 Berlin www.ibu-epd.com
Germany
Programme holder
Institut Bauen und Umwelt e.V. +49 (0)30 3087748- 0
Hegelplatz 1 info@ibu-epd.com
10117 Berlin www.ibu-epd.com
Germany
Author of the Life Cycle Assessment
Sphera Solutions GmbH +49 711 341817-0
Hauptstraße 111- 113 info@sphera.com
70771 Leinfelden-Echterdingen www.sphera.com
Germany
Owner of the Declaration
dormakaba International Holding GmbH +49 2333 793-0
DORMA Platz 1 info.de@dormakaba.com
58256 Ennepetal www.dormakaba.com
Germany
6 Environmental Product Declaration - Dormakaba - AL 401 Series Sliding Door Operator
