ENVIRONMENTAL PRODUCT DECLARATION
as per ISO 14025 and EN 15804+A2
Owner of the Declaration Knauf Ceiling Solutions GmbH & Co. KG
Publisher Institut Bauen und Umwelt e.V. (IBU)
Programme holder Institut Bauen und Umwelt e.V. (IBU)
Declaration number EPD-KNA-20210114-IBD2-EN
Issue date 25.05.2021
Valid to 24.05.2026
AMF ECOMIN & ARMSTRONG Basic Range; AMF THERMATEX &
ARMSTRONG Standard Range (Pontalier)
Knauf Ceiling Solutions GmbH & Co. KG
www.ibu-epd.com | https://epd-online.com
1. General Information
Knauf Ceiling Solutions GmbH & Co. KG AMF ECOMIN & ARMSTRONG Basic Range; AMF
THERMATEX & ARMSTRONG Standard Range
(Pontalier)
Programme holder Owner of the declaration
IBU – Institut Bauen und Umwelt e.V. Knauf Ceiling Solutions GmbH & Co. KG
Hegelplatz 1 Elsenthal 15
10117 Berlin 94481 Grafenau
Germany Germany
Declaration number Declared product / declared unit
EPD-KNA-20210114-IBD2-EN 1 m² THERMATEX/ARMSTRONG Standard Range mineral ceiling tiles
with an average surface weight of 3,25 kg/m².
This declaration is based on the product category rules: Scope:
Mineral panels, 01.08.2021 This document refers to 1 m² THERMATEX/ARMSTRONG Standard
(PCR checked and approved by the SVR) Range mineral ceiling tiles with an average recipe and an average surface
weight of 3,25 kg/m², manufactured at the production facility in Pontarlier,
France under the brand names THERMATEX and ARMSTRONG.
Issue date The owner of the declaration shall be liable for the underlying information
and evidence; the IBU shall not be liable with respect to manufacturer
25.05.2021
information, life cycle assessment data and evidences.
The EPD was created according to the specifications of EN 15804+A2. In
Valid to
the following, the standard will be simplified as EN 15804.
24.05.2026
Verification
The standard EN 15804 serves as the core PCR
Independent verification of the declaration and data according to ISO
14025:2011
internally X externally
Dipl.-Ing. Hans Peters
(Chairman of Institut Bauen und Umwelt e.V.)
Florian Pronold Prof. Dr. Birgit Grahl,
(Managing Director Institut Bauen und Umwelt e.V.) (Independent verifier)
Environmental Product Declaration - Knauf Ceiling Solutions GmbH & Co. KG - AMF ECOMIN & ARMSTRONG Basic Range; AMF THERMATEX & ARMSTRONG
1 Standard Range (Pontalier)
2. Product
The EPD refers to panels with a thickness between 12 - 19 mm
2.1 Product description/Product definition which can have variable length and width dimensions.
The ceiling tiles are manufactured using a wet felt process and
consist of biosoluble mineral wool, perlite, clay and starch. The 2.5 Base materials/Ancillary materials
ceiling tiles meet the requirements of DIN 18177 and EN
Mineral tile composition:
13964.
Name Value Unit
The AMF and Armstrong mineral tiles are available in a wide Mineral wool 5 - 60 %
range of different surface designs and product properties. Perlite 20 - 40 %
Depending on the design, the ceiling tiles are available in Clay 14 - 18 %
different formats and edge finishes.
Cellulose fibres 0 -12 %
Starch 4- 5 %
This EPD applies to the following products:
others 0 - 7 %
Basic Range: In addition, dispersion paints are used on the surface and water
Armstrong Bajkal, Armstrong Feria, Armstrong Savanna, for preparation during production. The recycled content is at
Armstrong Aleria L, Armstrong Atlas, Armstrong Retail, least 31 %.
Armstrong Scala, Armstrong Oasis, Armstrong Etna, ECOMIN
Orbit, ECOMIN Orbit micro, ECOMIN Planet, ECOMIN Filigran This product/article/at least one partial article contains
substances listed in the ECHA-candidate list (date: 25.06.2020)
Standard Range: exceeding 0.1 percentage by mass: No
Armstrong Bioguard Plain, Armstrong Plain, Armstrong Casa,
Armstrong Cortega, Armstrong Dune, Armstrong Dune NG, This product/article/at least one partial article contains other
Armstrong Dune eVo, Armstrong Dune eVo dB, Armstrong carcinogenic mutagenic reprotoxic (CMR) substances in
Dune Supreme, Armstrong Retail, Armstrong Sahara, categories 1A or 1B which are not on the candidate list,
Armstrong Sahara Max, Armstrong Tatra, Armstrong Fine exceeding 0.1 percentage by mass: No
Fissured, THERMATEX Schlicht, Star, THERMATEX Mercure,
THERMATEX Feinstratos, THERMATEX Feinstratos micro, Biocide products were added to this construction product or it
THERMATEX Fresko, THERMATEX Feinfresko has been treated with biocide products (this then concerns a
Please be aware of the limited representativity of the declared treated product as defined by the (EU) Ordinance on Biocide
impacts for the products Sahara A1 and Dune NG. For the Products No. 528/2012): No In-can preservatives are used in
placing on the market of the product in the European the production process; however, they are not part of the
Union/European Free Trade Association (EU/EFTA) (with the products and are therefore not within the scope of the
exception of Switzerland) Regulation (EU) No. 305/2011 (CPR) Ordinance on Biocide Products.
applies. The product needs a declaration of performance taking
into consideration EN 13964:2014, suspended ceiling Colemanite (2CaO – 3B2O3 – 5H2O) is used as a flame
requirements and test methods and the CE-marking. For the retardant in products with a reaction to fire A1 acc. to EN
application and use the respective national provisions apply. 13501-1 up to 6 % in the final product.
2.2 Application 2.6 Manufacture
Mineral tiles (wet-felt) are typically used as lay in for suspended The mineral tiles are produced in the traditional wet process
ceiling constructions. They are primarily used as optical (wet-felt). The raw materials are mixed with water to form a
cladding, but also for sound absorption and sound insulation, homogeneous suspension, which is pumped onto a belt
for fire resistance and against fire spreading, for cleanrooms conveyor (Fourdrinier). The water is removed mechanically
and high hygiene requirements. (gravity and vacuum) and by evaporation in the drying oven. As
far as possible, the process water is reused. It is treated
2.3 Technical Data
accordingly and fed back into the process water circuit.
Mineral boards (wet-felt) are regulated by EN 13964 and have
Depending on the desired appearance the panels can be
corresponding labelling and declaration of performance. The
sanded, colour-treated, patterned, eroded or embossed.
following data provide an overview of results:
Production waste and dust are reused in the process in the
Construction data (according to DIN 18177) sense of an internal cycle.
Name Value Unit The manufacturing plant is certified according to ISO 9001, ISO
14001 and OHSAS 18001.
Thermal conductivity 0.06 W/(mK)
Sound absorption coefficient acc. ISO 354 2.7 Environment and health during manufacturing
0.1 - 0.6 %
and ISO 11654 The manufacturer complies with all European regulations for
Airborne sound reduction acc. ISO 10848-2 the production of mineral slabs:
31 - 38 dB
and EN 717-1
Gross density 220 - kg/m3 • The manufacturing plant is certified according to ISO
280 9001, ISO 14001 and OHSAS 18001
Performance data of the product in accordance with the • The production has a closed water cycle, i.e. no waste
declaration of performance with respect to its essential water is produced
characteristics according to EN 13964:2014, suspended ceiling • Production generates virtually almost no waste, all
requirements and test methods (not part of CE-marking). resulting blanks, dust and rejects are reused to 99%
• Exclusive use of mineral fibres according to Regulation
2.4 Delivery status (EU) No.1272/2008 Note Q
Environmental Product Declaration - Knauf Ceiling Solutions GmbH & Co. KG - AMF ECOMIN & ARMSTRONG Basic Range; AMF THERMATEX & ARMSTRONG
2 Standard Range (Pontalier)
• Prohibition of the production and use of biopersistent Fire
fibres (Ordinance on Hazardous Substances, Annex II, The declared products are classified in the fire reaction class
No. 5) A2-s1, d0 according to EN 13501-1. This means that they are
• Prohibition of placing biopersistent fibres on the market "non-combustible" according to the German building authority
(Chemicals Prohibition Order, No.23 of the Annex to §1) designation (and also many other European countries) with
• Not subject to declaration according to REACH negligible smoke development and no burning drip in the event
of fire.
2.8 Product processing/Installation
Fire Reaction
There are no recognised systemic hazards associated with the
installation of ceiling tiles. It is recommended that materials are Name Value
handled in a manner that minimises dust generation. Workers Building material class A2
should wear appropriate personal protective equipment. Smoke gas development s1
Equipment such as gloves, goggles and dust masks are
Burning droplets d0
recommended to minimise exposure to dust and prevent skin
irritation.
Water
2.9 Packaging In the case of prolonged contact with water, the starch binder
The panels are packaged with cardboard boxes and sealed dissolves, which can lead to a loss of structure, and if the
with transparent polyethylene film.These packages lie on soluble components are discharged into the sewage treatment
chemically untreated wooden pallets. The pallets are wrapped plant, they are biodegradable, increasing the chemical oxygen
with polyethylene stretch film. Foil, paper and wood can be demand (COD) and the biological oxygen demand (BOD).
recycled in the usual ways.
Mechanical destruction
2.10 Condition of use The mineral slabs (wet-felt) can be broken by hand and also
When handled properly, the mechanical and structural-physical damaged superficially, which can result in dust formation.
properties of the mineral tile remain intact throughout its entire
service life. Direct contact with water should be avoided due to 2.14 Re-use phase
the water-soluble binding agent starch. If the panels are removed properly, they can be reinstalled. In
case of minor damage, the slabs can be reused as cut-to-size
2.11 Environment and health during use tiles. Mineral tiles can be returned to the manufacturing process
When properly installed, no dust/particles are released during if they are of the correct type and have sufficient material
the use phase. For the substance groups formaldehyde, volatile quality; they can be recycled up to 100 %.
organic compounds (VOCs) and total volatile organic
compounds (TVOCs), the limits according to DIN 18177 are 2.15 Disposal
complied with. The waste code number of production residues for mineral tiles
according to the AVV, German List of Wastes Ordinance is 10
2.12 Reference service life 11 03, the waste code number for construction site waste
The service life of the mineral tiles (wet-felted) is up to 50 (offcuts) is 17 06 04. If the tiles are not recycled as described in
years, depending on the area of use, exposure and state of 2.14., they are disposed of in a landfill.
maintenance. Within the framework of the conditions of use, no
ageing effects are to be expected apart from visual 2.16 Further information
discolouration caused by air circulation. Further information at www.knaufceilingsolutions.com
DoPs at knaufamf-dop.com or
2.13 Extraordinary effects www.knaufarmstrong.com/dop.html
3. LCA: Calculation rules
average composition of the raw boards, the recipe of each of
3.1 Declared Unit the products included in the average was considered.
This EPD refers to a declared unit of 1 m²
THERMATEX/Armstrong Standard Range ceiling tiles with an 3.2 System boundary
average surface weight of 3,25 kg/m². The life cycle assessment of average THERMATEX/Armstrong
Standard Range mineral ceiling tiles includes a cradle-to-gate
Declared unit
analysis of the products' environmental impacts with options.
Name Value Unit
Subsequent life cycle phases are part of the analysis:
Declared unit 1 m2
Grammage 3.25 kg/m2 Module A1–A3 | Production stage
The production stage includes the upstream burdens of raw
Layer thickness 0,014 m
material supply, their transports and the manufacturing plant of
conversion factor [Mass/Declared Unit] 3.25 -
Knauf Ceiling Solutions located in Pontarlier (France). Mineral
The ceiling tiles are produced at the Knauf Ceiling Solutions ceiling tiles are produced in the wet-felt process.
production site in Pontarlier, France under the brand names Main raw material inputs, therefore, refer to mineral wool,
THERMATEX and Armstrong. perlite, clay and starch. The production site is supplied with
electricity from the French power grid and thermal energy from
Various types of mineral ceiling tiles are produced at the site. A natural gas.
differentiation between the product groups was made based on
the recipe of the products. Standard products have common Module A4 | Transport from the gate to the site
product components and are manufactured in different Module A4 includes transport to the construction site. For this
thicknesses. The calculation of the weighted average recipe purpose, transport by truck over a distance of 470 km is used
and surface weight is based on the square meters produced of as a representative scenario.
each product. Ensuring the correct representation of the
Environmental Product Declaration - Knauf Ceiling Solutions GmbH & Co. KG - AMF ECOMIN & ARMSTRONG Basic Range; AMF THERMATEX & ARMSTRONG
3 Standard Range (Pontalier)
Module A5 | Assembly at the site This study uses generic background data for the evaluation of
For installation in the building, a scenario of 5 % loss is upstream environmental impacts from GaBi databases (GaBi
declared in this EPD. The losses during installation in the 10; 2020.2).
building are strongly dependent on the building geometry and
the specific application. Thus, the percentage of waste can vary 3.6 Data quality
greatly in the building context and must be adjusted accordingly Data collection is based on product-specific questionnaires. It
at the building level according to the actual conditions. In follows an iterative process clarifying questions via e-mail,
addition to the losses during installation in the building, Module telephone calls or in personal/web meetings. Intensive
A5 includes the environmental impacts from the End-of-Life of discussions between Knauf Ceiling Solutions and Daxner &
the packaging of the products. Merl results in an accurate mapping of product-related material
and energy flows. This leads to a high quality of foreground
Module C1 | Deconstruction and demolition data collected. Data collection relies on a consistent process
Disassembly of the product is done either manually or using according to ISO 14044.
smaller tools. Referring energy demand is considered to be
negligible. The weighted average was calculated based on the product-
specific recipes and composition. Its representativity is
Modul C2 | Transport to disposal considered to be good for 98 % of the THERMATEX/Armstrong
The transport to the disposal of the material is estimated Standard products.
declaring a 50 km radius to the landfill. In reality, this scenario
may vary depending on the actual location of deconstruction The technological, geographical and time-related
and referring waste treatment. representativeness of the database was kept in mind when
selecting background data. Whenever specific data were
Module C3 | Waste processing missing, either generic datasets or representative average data
The declared scenario assumes landfilling of the product. were used instead. The implemented GaBi background
Referring environmental impacts are accounted for in module datasets refer to the latest versions available (not more than
C4. ten years old) and are carefully chosen.
Module C4 | Disposal 3.7 Period under review
Module C4 refers to the emissions from the disposal of the Foreground data were collected in the 2019 production year,
mineral ceiling tiles. The chosen scenario, therefore, includes and the data are based on the volumes produced on an annual
the environmental burdens of landfilling of the product. basis.
3.8 Geographic Representativeness
Module D | Benefits and loads beyond the system
boundary Land or region, in which the declared product system is
The declared scenario assumes landfilling of the product. manufactured, used or handled at the end of the product´s
Referring environmental impacts are accounted for in module lifespan: France
C4. Module D declares the substitution potential from energy
recovery of the incineration of packaging waste in module A5.
3.9 Allocation
3.3 Estimates and assumptions All information for the allocation of given material and energy
flows is based on the site-related evaluations. The calculation
Assumptions and approximations are applied in case of a lack
of specific input quantities for the raw board production of the
of representative data. All assumptions and approximations are
analysed product group is based on the respective recipe. In
documented precisely and represent a best-guess
addition, product-specific application rates (e.g. basecoat, top
representation of reality. In case of uncertainty, a conservative
coat, etc.) were available for the upscaling of referring input
approach is chosen.
quantities. Total annual energy consumption and waste flows
3.4 Cut-off criteria are allocated based on the production share of each product.
The LCA model covers all available input and output flows,
which can be represented based on robust data. Data gaps are For in the production used waste paper, the system boundary is
filled with conservative assumptions from average data (when set after sorting. It is assumed that the end of waste status has
available) or with generic data and are documented been reached. Waste glass wool does not reach the end of
accordingly. Only data with a contribution lower 1 % were cut waste status. The system boundary for secondary raw
off. Thus, no data were neglected, of which a substantial impact materials defined in EN 15804 applies.
is to be expected. All relevant data were collected
3.10 Comparability
comprehensively. Cut-off material and energy flows were
Basically, a comparison or an evaluation of EPD data is only
chosen carefully based on their expected quantitative
possible if all the data sets to be compared were created
contribution as well as potential environmental impacts. Thus, it
according to EN 15804 and the building context, respectively
can be assumed that the sum of all neglected input flows does
the product-specific characteristics of performance, are taken
not account for more than 5 % of the total material, water and
into account. Zur Berechnung der Ökobilanz wurde die
energy flows.
-Hintergrunddatenbank verwendet
3.5 Background data
4. LCA: Scenarios and additional technical information
Information on the description of the biogenic carbon
Characteristic product properties of biogenic carbon
content at the factory gate
The biogenic carbon content quantifies the amount of biogenic
carbon in the declared product.
Environmental Product Declaration - Knauf Ceiling Solutions GmbH & Co. KG - AMF ECOMIN & ARMSTRONG Basic Range; AMF THERMATEX & ARMSTRONG
4 Standard Range (Pontalier)
Name ValueUnit End-of-Life (C1-C4)
kg
Biogenic carbon content in product 0.17 Name Value Unit
C
Collected separately 3.25 kg
Biogenic carbon content in accompanying kg
0.06 Landfilling 3.25 kg
packaging C
Transport to the site (A4)
Name Value Unit
Litres of fuel (fully loaded) 53 l/100km
Litres of fuel (empty) 14 l/100km
Transport distance 470 km
Capacity utilisation (including empty runs) 61 %
Gross density of products transported 207 kg/m3
Assembly (A5)
Name Value Unit
Packaging (cardboard) 0,02 kg/m²
Packaging (pallets) 0,12 kg/m²
Packaging (PE-foil) 0,01 kg/m²
Reference service life
Name Value Unit
Placing on the market according to
Declared product
EN 13964; see also document
properties (at the -
centre on the website
gate) and finishes
knaufceilingsolutions.com
Design application
parameters (if
instructed by the
manufacturer), See document centre on the
-
including the website knaufceilingsolutions.com
references to the
appropriate practices
and application codes
Indoor environment
The load classes of ceiling tiles
(for indoor
vary depending on the product,
applications), e.g.
from a fluctuating relative humidity -
temperature,
of 70 % at 25 °C up to 95 % at 30
moisture, chemical
°C, without corrosive impurities.
exposure
Usage conditions,
No mechanical stress during
e.g. frequency of use, -
conventional use.
mechanical exposure
As a rule, the ceiling tiles do not
Maintenance e.g.
need to be cleaned for the duration
required frequency,
of their use in normal application.
type and quality and -
However, the ceiling tiles can be
replacement of
cleaned dry and damp according to
components
the cleaning guideline.
Environmental Product Declaration - Knauf Ceiling Solutions GmbH & Co. KG - AMF ECOMIN & ARMSTRONG Basic Range; AMF THERMATEX & ARMSTRONG
5 Standard Range (Pontalier)
5. LCA: Results
The following table contains the LCA results for a declared unit of 1 m² average THERMATEX/Armstrong Standard Range mineral
ceiling tiles with an average surface weight of 3,25 kg/m².
DESCRIPTION OF THE SYSTEM BOUNDARY (X = INCLUDED IN LCA; ND = MODULE OR INDICATOR NOT DECLARED; MNR =
MODULE NOT RELEVANT)
Benefits and
Construction loads beyond
Product stage Use stage End of life stage
process stage the system
boundaries
la ire ta m w a Ry lp p u s tro p s n a rT g n iru tc a fu n a M e h t m o rf tro p s n a rTe tis e h t o t e ta g y lb m e s s A e s U e c n a n e tn ia M ria p e R tn e m e c a lp e R tn e m h s ib ru fe R y g re n e la n o ita re p Oe s u re ta w la n o ita re p Oe s u n o itc u rts n o c -e Dn o itilo m e d tro p s n a rT g n is s e c o rp e ts a W la s o p s iD -e s u e R-y re v o c e R-g n ilc y c e Rla itn e to p
A1 A2 A3 A4 A5 B1 B2 B3 B4 B5 B6 B7 C1 C2 C3 C4 D
X X X X X MND MND MNR MNR MNR MND MND X X X X X
RESULTS OF THE LCA - ENVIRONMENTAL IMPACT according to EN 15804+A2: 1 m² THERMATEX/Armstrong Standard Range
mineral ceiling tiles (3,25 kg/m²)
Parameter Unit A1-A3 A4 A5 C1 C2 C3 C4 D
GWP-total kg CO 2 eq 3.21E+00 9.11E-02 2.23E-01 0 9.69E-03 0 6.76E-01 -8.95E-03
GWP-fossil kg CO 2 eq 3.83E+00 9.23E-02 2.23E-01 0 9.82E-03 0 4.93E-02 -8.94E-03
GWP-biogenic kg CO 2 eq -6.26E-01 -2.26E-03 3.55E-05 0 -2.4E-04 0 6.27E-01 -1.11E-06
GWP-luluc kg CO 2 eq 2.2E-03 1.1E-03 1.17E-04 0 1.17E-04 0 1.42E-04 -2.61E-06
ODP kg CFC11 eq 8.75E-11 1.49E-17 4.38E-12 0 1.58E-18 0 1.83E-16 -6.96E-17
AP mol H+ eq 9.55E-03 3.29E-04 4.98E-04 0 3.5E-05 0 3.54E-04 -8.35E-06
EP-freshwater kg P eq 6.89E-05 6.35E-07 3.45E-06 0 6.76E-08 0 8.47E-08 -5.66E-09
EP-marine kg N eq 3.01E-03 1.44E-04 1.56E-04 0 1.53E-05 0 9.1E-05 -3.01E-06
EP-terrestrial mol N eq 3.34E-02 1.64E-03 1.73E-03 0 1.75E-04 0 1E-03 -3.2E-05
kg NMVOC
POCP 6.01E-03 2.79E-04 3.16E-04 0 2.97E-05 0 2.76E-04 -8.59E-06
eq
ADPE kg Sb eq 4.09E-07 8.63E-09 2.07E-08 0 9.18E-10 0 4.43E-09 -1.23E-09
ADPF MJ 7.4E+01 1.19E+00 3.74E+00 0 1.27E-01 0 6.47E-01 -2.58E-01
m3 world eq
WDP 1.37E-01 1.36E-03 9.76E-03 0 1.44E-04 0 5.17E-03 -5.52E-04
deprived
GWP = Global warming potential; ODP = Depletion potential of the stratospheric ozone layer; AP = Acidification potential of land and water; EP =
Eutrophication potential; POCP = Formation potential of tropospheric ozone photochemical oxidants; ADPE = Abiotic depletion potential for non-fossil
resources; ADPF = Abiotic depletion potential for fossil resources; WDP = Water (user) deprivation potential)
RESULTS OF THE LCA - INDICATORS TO DESCRIBE RESOURCE USE according to EN 15804+A2: 1 m²
THERMATEX/Armstrong Standard Range mineral ceiling tiles (3,25 kg/m²)
Parameter Unit A1-A3 A4 A5 C1 C2 C3 C4 D
PERE MJ 2.76E-01 9.69E-02 1.87E-02 0 1.03E-02 0 8.47E-02 -2.67E-02
PERM MJ 9.51E+00 0 4.76E-01 0 0 0 0 0
PERT MJ 9.79E+00 9.69E-02 4.94E-01 0 1.03E-02 0 8.47E-02 -2.67E-02
PENRE MJ 7.37E+01 1.2E+00 3.72E+00 0 1.28E-01 0 6.47E-01 -2.58E-01
PENRM MJ 3.8E-01 0 1.9E-02 0 0 0 0 0
PENRT MJ 7.4E+01 1.2E+00 3.74E+00 0 1.28E-01 0 6.47E-01 -2.58E-01
SM kg 4.38E-01 0 2.19E-02 0 0 0 0 0
RSF MJ 0 0 0 0 0 0 0 0
NRSF MJ 0 0 0 0 0 0 0 0
FW m3 3.55E-03 1.55E-04 2.48E-04 0 1.65E-05 0 1.63E-04 -6.29E-05
PERE = Use of renewable primary energy excluding renewable primary energy resources used as raw materials; PERM = Use of renewable primary
energy resources used as raw materials; PERT = Total use of renewable primary energy resources; PENRE = Use of non-renewable primary energy
excluding non-renewable primary energy resources used as raw materials; PENRM = Use of non-renewable primary energy resources used as raw
materials; PENRT = Total use of non-renewable primary energy resources; SM = Use of secondary material; RSF = Use of renewable secondary fuels;
NRSF = Use of non-renewable secondary fuels; FW = Use of net fresh water
RESULTS OF THE LCA – WASTE CATEGORIES AND OUTPUT FLOWS according to EN 15804+A2:
1 m² THERMATEX/Armstrong Standard Range mineral ceiling tiles (3,25 kg/m²)
Parameter Unit A1-A3 A4 A5 C1 C2 C3 C4 D
HWD kg 2.05E-06 1.5E-07 1.03E-07 0 1.6E-08 0 9.86E-09 -5.92E-11
NHWD kg 2.6E-01 2.56E-04 1.76E-01 0 2.72E-05 0 3.25E+00 -7.23E-05
RWD kg 4.22E-03 5.79E-06 2.12E-04 0 6.15E-07 0 7.35E-06 -4.67E-05
CRU kg 0 0 0 0 0 0 0 0
MFR kg 0 0 1.44E-01 0 0 0 0 0
MER kg 0 0 0 0 0 0 0 0
Environmental Product Declaration - Knauf Ceiling Solutions GmbH & Co. KG - AMF ECOMIN & ARMSTRONG Basic Range; AMF THERMATEX & ARMSTRONG
6 Standard Range (Pontalier)
EEE MJ 0 0 6.18E-02 0 0 0 0 0
EET MJ 0 0 1.1E-01 0 0 0 0 0
HWD = Hazardous waste disposed; NHWD = Non-hazardous waste disposed; RWD = Radioactive waste disposed; CRU = Components for re-use;
MFR = Materials for recycling; MER = Materials for energy recovery; EEE = Exported electrical energy; EET = Exported thermal energy
RESULTS OF THE LCA – additional impact categories according to EN 15804+A2-optional:
1 m² THERMATEX/Armstrong Standard Range mineral ceiling tiles (3,25 kg/m²)
Parameter Unit A1-A3 A4 A5 C1 C2 C3 C4 D
Disease
PM 1.08E-07 1.92E-09 5.65E-09 0 2.04E-10 0 4.38E-09 -7.07E-11
incidence
IR kBq U235 eq 1.04E+00 1.34E-03 5.19E-02 0 1.42E-04 0 7.55E-04 -1.19E-02
ETP-fw CTUe 2.39E+01 9.87E-01 1.22E+00 0 1.05E-01 0 3.7E-01 -6.86E-02
HTP-c CTUh 1.29E-09 2.21E-11 6.76E-11 0 2.35E-12 0 5.48E-11 -1.47E-12
HTP-nc CTUh 3.4E-08 1.43E-09 2E-09 0 1.52E-10 0 6.03E-09 -5.42E-11
SQP SQP 6.57E+01 8.45E-01 3.29E+00 0 8.99E-02 0 1.35E-01 -1.28E-02
PM = Potential incidence of disease due to PM emissions; IR = Potential Human exposure efficiency relative to U235; ETP-fw = Potential comparative
Toxic Unit for ecosystems; HTP-c = Potential comparative Toxic Unit for humans (cancerogenic); HTP-nc = Potential comparative Toxic Unit for humans
(not cancerogenic); SQP = Potential soil quality index
Disclaimer 1 – for the indicator “Potential Human exposure efficiency relative to U235”. This impact category deals mainly with the
eventual impact of low-dose ionizing radiation on human health of the nuclear fuel cycle. It does not consider effects due to possible
nuclear accidents, occupational exposure or radioactive waste disposal in underground facilities. Potential ionizing radiation from the
soil, radon and from some construction materials is also not measured by this indicator.
Disclaimer 2 – for the indicators “abiotic depletion potential for non-fossil resources”, “abiotic depletion potential for fossil resources”,
“water (user) deprivation potential, deprivation-weighted water consumption”, “potential comparative toxic unit for ecosystems”,
“potential comparative toxic unit for humans – cancerogenic”, “Potential comparative toxic unit for humans - not cancerogenic”,
“potential soil quality index”. The results of this environmental impact indicator shall be used with care as the uncertainties on these
results are high as there is limited experience with the indicator.
6. LCA: Interpretation
The following interpretation contains a summary of the LCA THERMATEX/Armstrong Standard Range mineral ceiling tiles.
results referenced to a functional unit of 1 m² average
Life of the products due to landfilling (module C4) have a minor
contribution.
The comparison of the product's life cycle phases shows a
clear dominance of the production phase (modules A1-A3) in all The direct emissions from the combustion of natural gas for the
environmental impact categories. The potential environmental production process represent the main driver when it comes to
impacts from transport to disposal (module C2) and the End-of- potential climate change (GWP) as well as depletion of fossil
Environmental Product Declaration - Knauf Ceiling Solutions GmbH & Co. KG - AMF ECOMIN & ARMSTRONG Basic Range; AMF THERMATEX & ARMSTRONG
7 Standard Range (Pontalier)
resources (ADPF). Potential acidification (AP), photooxidant of the products within the group shows a good representativity
creation (POCP) as well as terrestrial eutrophication (EP- of the results for 98 % of the production quantity. The
terrestrial) are dominated by direct emissions from natural gas environmental impacts of the product groups 12 mm, 15 Fiss,
combustion, the upstream supply chain of stone wool as well as 14 Sand, Sahara, Etna, ITP 13 mm, 14 Fiss, 15 Plain and 14
starch. Potential eutrophication of marine ecosystems (EP- Plain show <10 % variance except for ODP. For the 12 mm
marine) is mainly affected by upstream emission from starch boards, a potential overestimation of product-specific impacts
production and direct emissions at the site as well. When it between 10-30 % is to be expected.
comes to eutrophication potential of freshwater (EP-freshwater)
the share of the upstream supply chain of starch represents the The products Sahara A1 and Dune NG stand for more exotic
most dominant factor. Electricity from the French grid representatives of the Standard product group with a very low
represents an important driver when it comes to potential water production share. The declared average thus underestimates
scarcity (WDP). product-specific impacts with a variance between +70 % for
GWP until +200 % for ADP, leading to a limited representativity
The declared environmental impacts represent a weighted for A1 products.
average of the THERMATEX/Armstrong Standard product This can be traced back to a very high share of mineral wool in
group. The analysis of the variance of the specific composition the products.
7. Requisite evidence
7.1 Radioactivity
AgBB Overview (28 days)
Not applicable for these products.
Name Value Unit
7.2 Biopersistence TVOC (C6 - C16) 0,024 mg/m3
The mineral wool used for the production of the panels is TSVOC (C16 - C22) < 0,005 mg/m3
biosoluble and, according to EU Regulation 1272/2008/EC, is R (dimensionless) 0,0014
to be assessed as free of suspected cancer. "EUCEB"
VOC without NIK < 0,005 mg/m3
organization monitors and guarantees the quality of the wool
Carcinogenic substances < 0,001 mg/m3
used.
The production and use of non-exempt fibres is prohibited by
the Ordinance on Hazardous Substances and the Chemicals 7.4 Formaldehyde
Prohibition Ordinance. Measuring point: Eurofins Product Testing A/S
Test report: VOC emission test report Indoor Air Comfort GOLD
7.3 VOC emissions (08.02.2021)
Measuring point: Eurofins Product Testing A/S Number: 392-2020-00519909_A_EN
Test report: VOC emission test report Indoor Air Comfort GOLD Testing period: 17.11.2020-08.02.2021
(08.02.2021) Test basis: EN 16516
Number: 392-2020-00519909_A_EN The product complies with formaldehyde class E1 according to
Testing period: 17.11.2020-08.02.2021 EN 16516.
Test basis: ISO 16000-6, EN 16516
8. References
Standards into indoor air.
DIN 18177 ISO 354
DIN 18177:2012, Mineral tiles manufactured in the factory by DIN EN ISO 354:2003-12, Acoustics - Measurement of sound
the wet felt process - Characteristic values and test methods. absorption in reverberant rooms.
EN 13501-1 ISO 717-1
DIN EN 13501-1:2019, Classification of construction products DIN EN ISO 717-1:2013-06, Acoustics - Assessment of sound
and building elements according to their reaction to fire, Part 1: insulation in buildings and of building elements - Part 1:
Classification with the results of tests on the reaction to fire of Airborne sound insulation.
construction products.
ISO 9001
EN 13964 DIN EN ISO 9001:2015-11, Quality management systems -
DIN EN 13964:2014, Suspended ceilings - Requirements and Requirements.
test methods.
ISO 10848-2
EN 15804 DIN EN ISO 10848-2:2006-08, Acoustics - Measurement of
DIN EN 15804:2012+A2:2019, Sustainability of construction airborne and impact sound transmission between adjacent
works - Environmental product declarations - Core rules for the rooms in test stands - Part 2: Application to lightweight
product category of construction products. components where the connection has a minor influence.
EN 16487 ISO 11654
DIN EN 16487:2015-02, Acoustics - Test specifications for DIN EN ISO 11654:1997-07, Acoustics - Sound absorbers for
suspended ceilings - Sound absorption. use in buildings - Evaluation of sound absorption.
EN 16516 ISO 14001
DIN EN 16516:2020-10, Construction products: Assessment of DIN EN ISO 14001:2015-11, Environmental management
release of dangerous substances - Determination of emissions systems - Requirements with guidance for use.
Environmental Product Declaration - Knauf Ceiling Solutions GmbH & Co. KG - AMF ECOMIN & ARMSTRONG Basic Range; AMF THERMATEX & ARMSTRONG
8 Standard Range (Pontalier)
GaBi 10, Software-System and Database for Life Cycle
ISO 14025 Engineering. DB v8.7 2020.2. Stuttgart, Echterdingen: thinkstep
DIN EN ISO 14025:2011-10, Environmental labels and AG, 1992-2020. Available at: http://documentation.gabi-
declarations - Type III environmental declarations - Principles software.com.
and procedures.
IBU 2016
ISO 14044 Institut Bauen und Umwelt e.V.: General Programme
DIN EN ISO 14044:2006-10, Environmental management - Life Instructions for the Preparation of EPDs at the Institut Bauen
cycle assessment - Requirements and guidelines. und Umwelt e.V.. Version 1.1, Berlin: Institut Bauen und Umwelt
e.V., 2016. www.ibu-epd.com.
ISO 16000-6
ISO 16000-6:2011-12, Indoor air contaminants - Part 6: Ordinance on Biocide Products
Determination of VOCs in indoor air and test chambers, Regulation (EU) No 528/2012 of the European Parliament and
sampling on Tenax TA®, thermal desorption and gas of the Council of 22 May 2012 concerning the making available
chromatography with MS/FID. on the market and use of biocidal products.
OHSAS 18001 Ordinance on Hazardous Substances
OHSAS 18001-2007, Certification of occupational safety and Ordinance on Hazardous Substances, of 26 November 2010
health management systems. (Federal Law Gazette I p. 1643, 1644), last amended by Article
148 of the Law of 29 March 2017 (Federal Law Gazette I p.
Further References 626).
AgBB PCR Part A
Ausschuss zur gesundheitlichen Bewertung von Bauprodukte Institut Bauen und Umwelt e.V. (IBU), 2019. Product Category
(AgBB) (Committee for health-related evaluation of building Rules for Building-Related Products and Services. Part A:
products): Vorgehensweise bei der gesundheitlichen Calculation Rules for the Life Cycle Assessment and
Bewertung der Emissionen von flüchtigen organischen Requirements on the Project Report. Version 1.8.
Verbindungen (VOC und SVOC) aus Bauprodukten.
PCR: Mineral panels
AVV, German List of Wastes Ordinance Institut Bauen und Umwelt e.V. (IBU), 2019. Product Category
Regulation on the European Waste List. Rules for Building-Related Products and Services. Part B:
Requirements on the EPD for Mineral panels. Version 1.1.
Chemicals Prohibition Ordinance 10.12.2018.
Chemicals Prohibition Ordinance (German designation:
Chemikalien-Verbotsverordnung – ChemVerbotsV) of 20 REACH
January 2017 (Federal Law Gazette I p. 94; 2018 I p. 1389), Regulation (EC) No 1907/2006 of the European Parliament and
last amended by Article 300 of the Ordinance of 19 June 2020 Council from 18 December 2006, Regulation concerning the
(Federal Law Gazette I p. 1328). Registration, Evaluation, Authorisation and Restriction of
Chemicals (REACH).
ECHA-candidate list
List of substances of very high concern (SVHC) for Regulation (EU) Nr. 305/2011(CPR)
authorisation (ECHA Candidate List), 25.06.2020, published Regulation (EU) No 305/2011 of the European Parliament and
under Article 59 (10) of REACH. Helsinki: European Chemicals of the Council of 9 March 2011 laying down harmonised
Agency. conditions for the marketing of construction products and
repealing Council Directive 89/106/EEC Text with EEA
EUCEB relevance.
EUCEB, European Certification Board for Mineral Wool
Products. Brussels, Belgium. Regulation (EU) Nr.1272/2008
Regulation (EC) No 1272/2008 of the European Parliament and
Eurofins Product Testing A/S of the Council of 16 December 2008 on classification, labelling
Test report: VOC emission test report Indoor Air Comfort GOLD and packaging of substances and mixtures, amending and
(08.02.2021), Number: 392-2020-00519909_A_EN. repealing Directives 67/548/EEC and 1999/45/EC, and
amending Regulation (EC) No 1907/2006.
GaBi
Environmental Product Declaration - Knauf Ceiling Solutions GmbH & Co. KG - AMF ECOMIN & ARMSTRONG Basic Range; AMF THERMATEX & ARMSTRONG
9 Standard Range (Pontalier)
Publisher
Institut Bauen und Umwelt e.V. +49 (0)30 3087748- 0
Hegelplatz 1 info@ibu-epd.com
10117 Berlin www.ibu-epd.com
Germany
Programme holder
Institut Bauen und Umwelt e.V. +49 (0)30 3087748- 0
Hegelplatz 1 info@ibu-epd.com
10117 Berlin www.ibu-epd.com
Germany
Author of the Life Cycle Assessment
Daxner & Merl GmbH +43 676 849477826
Lindengasse 39/8 office@daxner-merl.com
1070 Wien www.daxner-merl.com
Austria
Owner of the Declaration
Knauf Ceiling Solutions GmbH & Co. KG 0049 8552 422 0
Elsenthal 15 info@knaufamf.com
94481 Grafenau www.knaufceilingsolutions.com
Germany
Environmental Product Declaration - Knauf Ceiling Solutions GmbH & Co. KG - AMF ECOMIN & ARMSTRONG Basic Range; AMF THERMATEX & ARMSTRONG
10 Standard Range (Pontalier)
