ver1 2015
ENVIRONMENTAL PRODUCT DECLARATION
in accordance with ISO 14025, ISO 21930 and EN 15804
Owner of the declaration: Vestre AS
Program operator: The Norwegian EPD Foundation
Publisher: The Norwegian EPD Foundation
Declaration number: NEPD-3028-1704-EN
Registration number: NEPD-3028-1704-EN
ECO Platform reference number: -
Issue date: 26.08.2021
Valid to: 26.08.2026
April Go chair wood
Vestre AS
www.epd-norge.no
NEPD-3028-1704-EN April Go chair wood 1 / 8
General information
Product: Owner of the declaration:
April Go chair wood
Vestre AS
Contact person: Øyvind Bjørnstad
Phone:
e-mail: ob@vestre.com
Program operator: Manufacturer:
Vestre AS
The Norwegian EPD Foundation
Pb. 5250 Majorstuen, 0303 Oslo
Phone: +47 23 08 80 00
e-mail: post@epd-norge.no
Declaration number: Place of production:
Vestre AS
NEPD-3028-1704-EN Drammensveien 44A 0271 Oslo
Norway
ECO Platform reference number: Management system:
ISO 14001:2015, Cert nr. 1422367 and ISO 9001: 2015, Cert nr. 32147
This declaration is based on Product Category Rules: Organisation no:
948 140 349
CEN Standard EN 15804:2012+A1:2013 serves as core PCR
NPCR 026:2018 Part B for furniture
Statement of liability: Issue date: 26.08.2021
The owner of the declaration shall be liable for the underlying information and
evidence. EPD Norway shall not be liable with respect to manufacturer Valid to: 26.08.2026
information, life cycle assessment data and evidences.
Declared unit: Year of study:
1 Pcs April Go chair wood 2020
Declared unit with option: Comparability:
A1,A2,A3,A4,A5,C1,C2,C3,C4,D EPDs from programmes other than the Norwegian EPD Foundation may not be
comparable
Functional unit: Development and verification of EPD:
The declaration has been developed and verified using EPD tool lca.tools
ver EPD2020.11, developed by LCA.no AS. The EPD tool is integrated into
the company's environmental management system, and has been
approved by EPD-Norway
General information on verification of EPD from EPD tools:
Independent verification of data, other environmental information and Developer of EPD:
the declaration according to ISO 14025:2010, § 8.1.3 and § 8.1.4. Individual
third party verification of each EPD is not required when the EPD tool is i) Øyvind Bjørnstad
integrated into the company's environmental management system, ii) the
procedures for use of the EPD tool are approved by EPDNorway, and iii) Reviewer of company-specific input data and EPD:
the proccess is reviewed annualy. See Appendix G of EPD-Norway's
General Programme Instructions for further information on EPD tools. Michaela Båtnäs
Verification of EPD tool: Approved:
Independent third party verification of the EPD tool, background data
Sign
and test-EPD in accordance with EPDNorway's procedures and guidelines
for verification and approval of EPD tools.
Erik Svanes, Norsus AS
(no signature required) Håkon Hauan, CEO EPD-Norge
Key environmental indicators Unit Cradle to gate A1 - A3
Global warming kg CO2 eqv 29,65
Total energy use MJ 448,23
Amount of recycled materials % 2,30
NEPD-3028-1704-EN April Go chair wood 2 / 8
Product
Market: Technical data:
Global
Product description: Reference service life, product
APRIL GO chair is available with or without armrests, and can be
50 years
stacked and moved as required. Its sturdy construction makes it
difficult to knock over and reduces the risk of it being removed by Reference service life, building
unauthorised persons. The APRIL GO chair can be supplied with a
practical storage trolley with space for eight chairs.
Product specification
Recycled share in Recycled share in
Materials kg %
material (kg) material (%)
Metal - Steel 8,50 79,72 0,22 2,60
Metal - Zinc 0,51 3,68 0,00 0,00
Wood - Solid pine 2,14 15,44 0,00 0,06
Powder coating 0,16 1,17 0,00 0,00
Recycled share in Recycled share in
Packaging kg
material (kg) material (%)
Packaging - Cardboard 0,10 0,08 76,30
Packaging - Pallet 1,56 0,00 0,00
Packaging - Plastic 0,05 0,00 0,00
LCA: Calculation rules
Declared unit: Allocation:
The allocation is made in accordance with the provisions of EN 15804. Effects
1 Pcs April Go chair wood
of primary production of recycled materials is allocated to the main product
Cut-off criteria: in which the material was used. The recycling process and transportation of
the material is allocated to this analysis.
All major raw materials and all the essential energy is included. The
production processes for raw materials and energy flows with very small Where virgin materials are used, emissions and energy consumption
amounts (less than 1%) are not included. These cut-off criteria do not connected with extraction and production are included.
apply for hazardous materials and substances. Where recycled materials are used in the product, emissions and energy
consumption related to the recycling process are included.
Emissions from incineration are allocated to the product system that uses the
recovered energy.
Emissions from incineration of waste are allocated to the product system that
uses the recovered energy.
Data quality:
Specific data for the product composition are provided by the manufacturer. They represent the production of the declared product and were collected for
EPD development in the year of study. Background data is based on registered EPDs according to EN 15804, Ostfold Research databases, ecoinvent and other
LCA databases. The data quality of the raw materials in A1 is presented in the table below.
Specific manufacturing data are used. Raw materials by and large using EPD data, except for minor items like nuts & screws which are based on databases.
Materials Source Data quality Year
Metal - Zinc ecoinvent 3.4 Database 2017
Packaging - Cardboard ecoinvent 3.4 Database 2017
Packaging - Plastic ecoinvent 3.4 Database 2017
Packaging - Pallet Modified ecoinvent 3.4 Database 2017
Powder coating ecoinvent 3.5 Database 2018
Average (NEPD-474-330, NEPD-1808-766, NEPD-1818-767 and
Wood - Solid pine EPD 2020
NEPD-2196-1003)
Metal - Steel S-P-01919 EPD 2020
NEPD-3028-1704-EN April Go chair wood 3 / 8
System boundary:
Life cycle stages included are described in the figure and through the corresponding letter and number designations in the declaration (see figure below).
Additional technical information:
NEPD-3028-1704-EN April Go chair wood 4 / 8
The following information describe the scenarios in the different modules of the EPD.
The following information describe the scenarios in the different modules of the EPD.
Transportation to an average customer in Paris, France is 1,850 km (A4: average Euro 6 lorry > 32 tonnes). The use stage is not represented currently, as it
varies very much, although the furniture as a rule require very little maintenance. End of life is represented by a dismantling and recycling of metals, whilst
wood currently is being sent to incineration. We aim to change this as well.
Transport from production place to user (A4)
Capacity utilisation Fuel/Energy
Type Type of vehicle Distance km Unit Value (l/t)
(incl. return) % consumption
Truck 55,0 % Truck, over 32 tonnes, EURO 6 1850 0,022606 l/tkm 41,82
Railway l/tkm
Boat l/tkm
Other Transportation l/tkm
Assembly (A5) End of Life (C1, C3, C4)
. Unit Value . Unit Value
Auxiliary kg Hazardous waste disposed kg
Water consumption m3 Collected as mixed construction waste kg
Electricity consumption kWh Reuse kg
Other energy carriers MJ Recycling kg
Material loss kg Energy recovery kg 2,1400
Output materials from waste treatment kg 0,1480 To landfill kg 0,1096
Dust in the air kg
VOC emissions kg
Transport to waste processing (C2)
Capacity utilisation Fuel/Energy
Type Type of vehicle Distance km Unit Value (l/t)
(incl. return) % consumption
Truck 38,8 % Truck, 16-32 tonnes, EURO 6 500 0,043626 l/tkm 21,81
Railway l/tkm
Boat l/tkm
Other Transportation l/tkm
¨
Benefits and loads beyond the system boundaries (D)
. Unit Value
Substitution of electricity, in Norway (MJ) MJ 3,76
Substitution of thermal energy, district heating, in Norway (MJ) MJ 31,43
Substitution of primary construction steel, with net scrap steel (kg) kg 8,19
NEPD-3028-1704-EN April Go chair wood 5 / 8
LCA: Results
The LCA results are presented below for the declared unit defined on page 2 of the EPD document.
System boundaries (X=included, MND=module not declared, MNR=module not relevant)
Construction Beyond the
Product stage installation User stage End of life stage . system
stage bondaries
A1 A2 A3 A4 A5 B1 B2 B3 B4 B5 B6 B7 C1 C2 C3 C4 . D
X X X X X MND MND MND MND MND MND MND X X X X . X
Environmental impact
Parameter Unit A1 A2 A3 A4 A5
GWP kg CO 2 -eq 2,86E+01 6,22E-01 3,84E-01 1,99E+00 2,13E-01
ODP kg CFC11 -eq 3,20E-07 1,17E-07 2,55E-07 4,09E-07 7,68E-09
POCP kg C 2H 4-eq 9,40E-03 9,41E-05 8,80E-05 3,12E-04 1,55E-05
AP kg SO 2 -eq 8,03E-02 1,46E-03 2,31E-03 5,15E-03 4,11E-04
EP kg PO 3- -eq 1,67E-02 1,92E-04 5,28E-04 7,10E-04 1,09E-04
4
ADPM kg Sb -eq 3,68E-03 1,93E-06 2,82E-06 4,75E-06 1,14E-07
ADPE MJ 3,18E+02 9,38E+00 4,27E+00 3,27E+01 8,40E-01
Parameter Unit C1 C2 C3 C4 D
GWP kg CO 2 -eq 0 1,04E+00 3,27E+00 1,60E-03 -1,40E+01
ODP kg CFC11 -eq 0 1,95E-07 2,35E-08 2,56E-10 -6,30E-07
POCP kg C 2H 4-eq 0 1,57E-04 2,70E-05 2,87E-07 -9,84E-03
AP kg SO 2 -eq 0 2,44E-03 6,83E-04 6,64E-06 -6,26E-02
EP kg PO 3- -eq 0 3,20E-04 1,83E-04 1,14E-06 -2,08E-02
4
ADPM kg Sb -eq 0 3,22E-06 3,58E-07 1,71E-10 -2,67E-04
ADPE MJ 0 1,57E+01 1,95E+00 2,28E-02 -1,32E+02
GWP Global warming potential; ODP Depletion potential of the stratospheric ozone layer; POCP Formation potential of tropospheric photochemical oxidants;
AP Acidification potential of land and water; EP Eutrophication potential; ADPM Abiotic depletion potential for non fossil resources; ADPE Abiotic depletion
potential for fossil resources
Reading example: 9,0 E-03 = 9,0*10-3 = 0,009
*INA Indicator Not Assessed
waR slairetam tropsnarT gnirutcafunaM tropsnarT ylbmessA esU ecnanetniaM riapeR tnemecalpeR tnemhsibrufeR lanoitarepO ygrene esu lanoitarepO esu
retaw
-eD noitcurtsnoc noitilomed tropsnarT etsaW gnissecorp lasopsiD -yrevoceR-esueR -gnilcyceR laitnetop
NEPD-3028-1704-EN April Go chair wood 6 / 8
Resource use
Parameter Unit A1 A2 A3 A4 A5
RPEE MJ 6,48E+01 1,39E-01 1,33E+01 5,95E-01 2,35E+01
RPEM MJ 6,86E+01 0,00E+00 0,00E+00 0,00E+00 0,00E+00
TPE MJ 1,33E+02 1,39E-01 1,33E+01 5,95E-01 2,35E+01
NRPE MJ 3,28E+02 9,61E+00 3,23E+01 3,38E+01 2,89E+00
NRPM MJ 3,56E+00 0,00E+00 0,00E+00 0,00E+00 0,00E+00
TRPE MJ 3,32E+02 9,61E+00 3,23E+01 3,38E+01 2,89E+00
SM kg 3,66E-01 0,00E+00 0,00E+00 0,00E+00 0,00E+00
RSF MJ 1,17E-02 0,00E+00 1,27E-02 0,00E+00 0,00E+00
NRSF MJ 7,81E-03 0,00E+00 0,00E+00 0,00E+00 0,00E+00
W m3 2,19E-01 1,82E-03 7,80E-03 7,99E-03 7,58E-04
Parameter Unit C1 C2 C3 C4 D
RPEE MJ 0 2,31E-01 3,24E-02 7,10E-04 -2,64E+01
RPEM MJ 0 0,00E+00 0,00E+00 0,00E+00 0,00E+00
TPE MJ 0 2,31E-01 3,24E-02 7,10E-04 -2,64E+01
NRPE MJ 0 1,60E+01 2,01E+00 2,38E-02 -1,31E+02
NRPM MJ 0 0,00E+00 0,00E+00 0,00E+00 0,00E+00
TRPE MJ 0 1,60E+01 2,01E+00 2,38E-02 -1,31E+02
SM kg 0 0,00E+00 0,00E+00 0,00E+00 0,00E+00
RSF MJ 0 0,00E+00 0,00E+00 0,00E+00 -7,40E-04
NRSF MJ 0 0,00E+00 0,00E+00 0,00E+00 0,00E+00
W m3 0 3,03E-03 8,36E-04 2,42E-05 -8,62E-02
RPEE Renewable primary energy resources used as energy carrier; RPEM Renewable primary energy resources used as raw materials; TPE Total use of renewable
primary energy resources; NRPE Non renewable primary energy resources used as energy carrier; NRPM Non renewable primary energy resources used as
materials; TRPE Total use of non renewable primary energy resources; SM Use of secondary materials; RSF Use of renewable secondary fuels; NRSF Use of non
renewable secondary fuels; W Use of net fresh water
Reading example: 9,0 E-03 = 9,0*10-3 = 0,009
*INA Indicator Not Assessed
End of life - Waste
Parameter Unit A1 A2 A3 A4 A5
HW kg 3,64E-02 5,66E-06 1,21E-05 1,80E-05 1,33E-06
NHW kg 4,41E+00 5,15E-01 2,60E-01 3,08E+00 7,21E-02
RW kg INA* INA* INA* INA* INA*
Parameter Unit C1 C2 C3 C4 D
HW kg 0 9,45E-06 5,22E-06 3,29E-08 -1,19E-03
NHW kg 0 8,59E-01 1,04E-01 1,15E-01 -2,36E+01
RW kg 0 INA* INA* INA* INA*
HW Hazardous waste disposed; NHW Non hazardous waste disposed; RW Radioactive waste disposed
Reading example: 9,0 E-03 = 9,0*10-3 = 0,009
*INA Indicator Not Assessed
End of life - Output flow
Parameter Unit A1 A2 A3 A4 A5
CR kg 0,00E+00 0,00E+00 0,00E+00 0,00E+00 0,00E+00
MR kg 4,31E-03 0,00E+00 3,00E+00 0,00E+00 0,00E+00
MER kg 1,79E-02 0,00E+00 2,28E-04 0,00E+00 0,00E+00
EEE MJ INA* INA* INA* INA* INA*
ETE MJ INA* INA* INA* INA* INA*
Parameter Unit C1 C2 C3 C4 D
CR kg 0 0,00E+00 0,00E+00 0,00E+00 0,00E+00
MR kg 0 0,00E+00 8,42E+00 0,00E+00 0,00E+00
MER kg 0 0,00E+00 2,14E+00 0,00E+00 0,00E+00
EEE MJ 0 INA* INA* INA* INA*
ETE MJ 0 INA* INA* INA* INA*
CR Components for reuse; MR Materials for recycling; MER Materials for energy recovery; EEE Exported electric energy; ETE Exported thermal energy
Reading example: 9,0 E-03 = 9,0*10-3 = 0,009
*INA Indicator Not Assessed
NEPD-3028-1704-EN April Go chair wood 7 / 8
Additional Norwegian requirements
Greenhouse gas emissions from the use of electricity in the manufacturing phase
National production mix from import, low voltage (production of transmission lines, in addition to direct emissions and losses in grid) of applied electricity for the manufacturing
process (A3).
Electricity mix Data source Amount Unit
El-mix, Sweden (kWh) ecoinvent 3.4 Alloc Rec 42,67 g CO2-ekv/kWh
Dangerous substances
The product contains no substances given by the REACH Candidate list or the Norwegian priority list.
Indoor environment
Vestre recommends oak or ash if the product contains wood and is intended for indoor use.
Additional environmental information
Bibliography
ISO 14025:2010 Environmental labels and declarations - Type III environmental declarations - Principles and procedures.
ISO 14044:2006 Environmental management - Life cycle assessment - Requirements and guidelines.
EN 15804:2012+A1:2013 Environmental product declaration - Core rules for the product category of construction products.
ISO 21930:2017 Sustainability in buildings and civil engineering works - Core rules for environmental product declarations of construction products.
ecoinvent v3, Allocation, cut-off by classification, Swiss Centre of Life Cycle Inventories.
Iversen et al., (2018) eEPD v3.0 - Background information for EPD generator system. LCA.no report number 04.18
Vold et al., (2019) EPD generator for Norsk Industri, Background information for industry application and LCA data, LCA.no report number 06.19.
NPCR Part A: Construction products and services. Ver. 1.0. April 2017, EPD-Norge.
NPCR 026 Part B for Furniture. Ver. 2.0 October 2018, EPD-Norge.
Program operator and publisher Phone: +47 23 08 80 00
The Norwegian EPD Foundation e-mail: post@epd-norge.no
Post Box 5250 Majorstuen, 0303 Oslo,Norway web: www.epd-norge.no
Owner of the declaration Phone:
Vestre AS e-mail: ob@vestre.com
Drammensveien 44A 0271 Oslo web: vestre.com
Author of the Life Cycle Assessment Phone: +47 916 50 916
LCA.no AS e-mail: post@lca.no
Dokka 1C 1671 Kråkerøy web: www.lca.no
Developer of EPD generator Phone: +47 916 50 916
LCA.no AS e-mail: post@lca.no
Dokka 1C 1671 Kråkerøy web: www.lca.no
NEPD-3028-1704-EN April Go chair wood 8 / 8
