Environmental product declaration
in accordance with ISO 14025 and EN 15804+A2
Arena 1700
Owner of the declaration: Program operator:
SG Armaturen AS The Norwegian EPD Foundation
Product: Declaration number:
Arena 1700
NEPD-8945-8608
Declared unit:
1 pcs
Registration number:
This declaration is based on Product Category Rules: NEPD-8945-8608
CEN Standard EN 15804:2012+A2:2019 serves as core
Issue date: 04.02.2025
PCR
The Norwegian EPD Foundation IBU PCR - Part B for luminaires, lamps, and components Valid to: 04.02.2030
for luminaires
EPD software:
LCAno EPD generator ID: 780766
1 / 14
General information
Product Owner of the declaration:
Arena 1700 SG Armaturen AS
Contact person: Audun Skare
Phone: +47 90021243
e-mail: audun.skare@sg-as.no
Program operator: Manufacturer:
The Norwegian EPD Foundation SG Armaturen AS
Post Box 5250 Majorstuen, 0303 Oslo, Norway Skytterheia 25
Phone: +47 977 22 020 4790 Lillesand, Norway
web: www.epd-norge.no
Declaration number: Place of production:
SG Armaturen production site Odense (Denmark
NEPD-8945-8608
Egestubben 26
5270 Odense, Denmark
This declaration is based on Product Category Rules: Management system:
CEN Standard EN 15804:2012+A2:2019 serves as core PCR
IBU PCR - Part B for luminaires, lamps, and components for
luminaires
Statement of liability: Organisation no:
The owner of the declaration shall be liable for the underlying 958560931
information and evidence. EPD Norway shall not be liable with respect
to manufacturer information, life cycle assessment data and
evidences.​
Declared unit: Issue date: 04.02.2025
1 pcs Arena 1700
Declared unit with option: Valid to: 04.02.2030
A1,A2,A3,A4,A5,B6,C1,C2,C3,C4,D
Year of study:
2021
Functional unit: Comparability:
1 Arena 1700 LED luminaire manufactured and installed, used EPD of construction products may not be comparable if they not
according to a specific lighting regime over 15 years, including waste comply with EN 15804 and seen in a building context.
treatment at end-of-life
General information on verification of EPD from EPD tools: Development and verification of EPD:
Independent verification of data, other environmental information The declaration is created using EPD tool lca.tools ver EPD2021.09,
and the declaration according to ISO 14025:2010, § 8.1.3 and § 8.1.4. developed by LCA.no. The EPD tool is integrated in the company's
Verification of each EPD is made according to EPD-Norway’s management system, and has been approved by EPD Norway.
guidelines for verification and approval requiring that tools are i) NEPDT63
integrated into the company's environmental management system, ii)
the procedures for use of the EPD tool are approved by EPD-Norway, Developer of EPD: Benedikte Ruud Andersen
and iii) the process is reviewed annually by an independent third
Reviewer of company-specific input data and EPD:​ Audun Skare
party verifier. See Appendix G of EPD-Norway's General Programme
Instructions for further information on EPD tools
Verification of EPD tool: Approved:
Independent third party verification of the EPD tool, background data
and test-EPD in accordance with EPDNorway's procedures and
guidelines for verification and approval of EPD tools. Approval
number: NEPDT41.
Third party verifier:
Vito D’Incognito, Take Care International
(no signature required)
2 / 14
Product
Product description:
Energy efficient surface mounted IP23 luminaire for use in industry and storage. It is easy to install with hinged gear tray, and can be mounted
either direct on ceiling (screws) or by using the mounting hooks for horizontal wiring. It is available in two lengths and with threee different light
distributions.
Wattage: 113W. Luminous flux: 16830lm. Efficacy: 149 lm/W. Colour temperature: 4000K. Colour rendering: Ra>80. Housing: Sheet steel. Colour:
White (RAL 9010, 20% gloss). Dimensions: 1842 x 137 x 59 mm. EAN: 5703821178440.
The EPD also covers the following product:
EAN: 5703821178167 - Arena 1500 White Wide 11800lm 4000K Ra>80 On/Off
Product specification
Materials kg %
Coating materials 0,22 3,92
Electronic - Connector 0,03 0,44
Electronic - LED chip 0,00 0,07
Electronic - LED driver 0,29 5,04
Electronic - LED plate 0,29 5,19
Electronic - Wire 0,25 4,32
Plastic - Plexiglass (PMMA) 0,64 11,33
Plastic - Polyethylene (HDPE) 0,00 0,07
Metal - Steel 3,96 69,62
Total 5,68 100,00
Packaging kg %
Packaging - Cardboard 0,20 100,00
Total incl. packaging 5,88 100,00
Technical data:
Link to the CE Declaration on our website:
https://www.sg-as.com/storage/data/130073_Arena/50/130073_Arena.pdf
Link to product data on our website:
https://www.sg-as.com/products/arena/8246094801
Market:
Nordic + Northwestern Europe.
Reference service life, product
15 years. Estimated based on the characteristics of the product and the intended application.
Reference service life, building or construction works
60 years. Standard service life for buildings according to the PCR Part A of EPD Norway.
LCA: Calculation rules
Declared unit:
1 pcs Arena 1700
Cut-off criteria:
All major raw materials and all the essential energy is included. The production processes for raw materials and energy flows with very small
amounts (less than 1%) can be excluded. These cut-off criteria do not apply for hazardous materials and substances.
Allocation:
The allocation is made in accordance with the provisions of EN 15804. Incoming energy and water and waste production in-house is allocated
equally among all products through mass allocation. Effects of primary production of recycled materials is allocated to the main product in which
the material was used. The recycling process and transportation of the material is allocated to this analysis.
Data quality:
Specific data for the product composition are provided by the manufacturer. The data represent the production of the declared product and were
collected for EPD development in the year of study. Background data is based on EPDs according to EN 15804 and different LCA databases. The
data quality of the raw materials in A1 is presented in the table below.
3 / 14
Materials Source Data quality Year
Coating materials ecoinvent 3.6 Database 2019
Electronic - Connector ecoinvent 3.6 Database 2019
Scientific
Electronic - LED chip Scholand et al. (2012) + Ecoinvent 3.6 literature + 2017
database
Supplier data +
Electronic - LED driver Material composition + ecoinvent 3.6 2019
database
Electronic - LED plate ecoinvent 3.6 Database 2019
Supplier data +
Electronic - Wire Material composition + ecoinvent 3.6 2019
database
Metal - Steel ecoinvent 3.6 Database 2019
Metal - Steel SG Armaturen + ecoinvent 3.6 Database 2019
Packaging - Cardboard ecoinvent 3.6 Database 2019
Plastic - Plexiglass (PMMA) ecoinvent 3.6 Database 2019
Plastic - Polyethylene (HDPE) ecoinvent 3.6 Database 2019
4 / 14
System boundaries (X=included, MND=module not declared, MNR=module not relevant)
Construction Beyond the system
Product stage Use stage End of life stage
installation stage boundaries
A1 A2 A3 A4 A5 B1 B2 B3 B4 B5 B6 B7 C1 C2 C3 C4 D
X X X X X MND MND MND MND MND X MND X X X X X
System boundary:
Additional technical information:
Link to the user manual on our website, for proper use of the product:
https://www.sg-as.com/storage/data/130073_Arena/20/5703821178440_Arena%201700_User%20Manual.pdf
waR slairetam tropsnarT gnirutcafunaM tropsnarT ylbmessA e​sU ecnanetniaM riapeR tnemecalpeR tnemhsibrufeR lanoitarepO ygrene esu lanoitarepO esu retaw -eD noitcurtsnoc noitilomed tropsnarT etsaW gnissecorp lasopsiD -yrevoceR-esueR laitnetop-gnilcyceR
5 / 14
LCA: Scenarios and additional technical information
The following information describe the scenarios in the different modules of the EPD.
Module A4 = Transportation is done by truck (1000 km) from the production site in Odense, Denmark to the warehouse in Lillesand, Norway or
to the warehouse in Mechelen, Belgium + 800 km for Nordic / Northwestern Europe Market.
Module A5 = Installation is performed in the Nordic / Northwestern Europe Market and done by manual labor, with the use of electrical machines,
that fall under the cut-off criteria of 1% and is therefore neglected. Packaging of the final product consist of a corrugated board box.
Module B6 = The operational energy use of the luminaire is calculated based on the methodology provided in IBU PCR Part B for luminaires,
lamps, and components for luminaires. The energy consumption model for luminaire used in the PCR follows the application scenarios developed
in EN 15193:2007. To calculate the electricity use of the luminaire, the following scenario parameters have been applied:
- Scenario: Sport
- Active power of the luminaire (Pa) = 113 watt
- Passive power of the luminaire (Pp) = 0 watt
- Daylight time usage (tD) = 2000 hours
- Non-daylight time usage (tN) = 2000 hours
- Standard year time (ty) = 8760 hours
- The occupancy depency factor (FO) = 1
- The daylight dependency factor (FD) = 1
- The product specific constant illuminance factor (FCP) = 1
- The non-daylight dimming factor (FN) = 1
- The application specific empiric lifetime of the luminaire in years (a) = 15 years (corresponding to the reference service life of the product).
Module C1 = The de-installation of the luminaire is done by manual labor, with the help of electrical machines. The use of portable electrical
devices (e.g., drill) usually have low energy requirements falling under the cut-off-criterion of 1% and is therefore neglected.
Module C2 = Transportation from building site to the waste treatment facility with an average distance of 300km.
Modules C3 and C4 = Waste treatment of the product follows the default values provided in EN 50693, Product Category Rules for life cycle
assessments of electronic and electrical products and systems, table G.4. This table specified how different types of raw materials used in A1 will
likely be treated during the end-of-life of the product. Waste treatments in C3 include material recycling and incineration with and without energy
recovery and fly ash extraction. Disposal in C4 consist of landfilling of different waste fractions and of ashes.
Module D = The recyclability of metals, plastics, and electronic components allows the producers a credit for the net scrap that is produced at the
end of a product’s life. The benefits from recycling of net scrap are described in formula from EN 15804:2012+A2:2019. Substitution of heat and
electricity generated by the incineration with energy recovery of plastic insulation and other parts is also calculated in module D.
Capacity utilisation Value
Transport from production place to user (A4) Distance (km) Fuel/Energy Consumption Unit
(incl. return) % (Liter/tonne)
Truck, 16-32 tonnes, EURO 6 (km) 36,7 % 900 0,043 l/tkm 38,70
Assembly (A5) Unit Value
Waste, cardboard and paper, to average treatment
kg 0,20
- A5 including transport (kg)
Operational energy (B6) Unit Value
Electricity, Norway (kWh) kWh/DU 6780,000000000
Capacity utilisation Value
Transport to waste processing (C2) Distance (km) Fuel/Energy Consumption Unit
(incl. return) % (Liter/tonne)
Truck, 16-32 tonnes, EURO 6 (km) 36,7 % 300 0,043 l/tkm 12,90
6 / 14
Waste processing (C3) Unit Value
Waste treatment of plastic mixture, incineration
kg 0,42
with energy recovery and fly ash extraction (kg)
Waste treatment per kg used electronic
kg 0,24
components, manual seperation (kg)
Copper to recycling (kg) kg 0,078
Steel to recycling (kg) kg 3,21
Waste treatment per kg used electronic plug
kg 0,025
connector, manual seperation (kg)
Waste treatment of polyethylene (PE),
incineration with energy recovery and fly ash kg 0,0021
extraction (kg)
Waste treatment of hazardous waste, incineration
kg 0,22
with fly ash extraction (kg)
Waste treatment per kg used PWB, shredding and
kg 0,45
separation - C3 (kg)
Waste treatment per kg electronics scrap from
PWB, with components, recycling of metals C3 kg 0,080
(kg)
Waste treatment per kg used electronic LED driver,
kg 0,28
manual seperation (kg)
Waste treatment per kg electronics scrap from
PWB, without components, recycling of copper - kg 0,14
C3 (kg)
Disposal (C4) Unit Value
Landfilling of ashes from incineration of Plastic
kg 0,014
mixture, process per kg ashes and residues (kg)
Landfilling of plastic mixture (kg) kg 0,42
Landfilling of copper (kg) kg 0,052
Landfilling of steel (kg) kg 0,80
Landfilling of ashes from incineration of
Polyethylene (PE), process per kg ashes and kg 0,000074
residues (kg)
Landfilling of ashes from incineration of
Hazardous waste, process per kg ashes and kg 0,042
residues - C4 (kg)
Landfilling of hazardous waste (kg) kg 0,23
Benefits and loads beyond the system
Unit Value
boundaries (D)
Substitution of electricity (MJ) MJ 0,65
Substitution of thermal energy, district heating
MJ 9,93
(MJ)
Substitution of primary copper with net scrap (kg) kg 0,056
Substitution of primary steel with net scrap (kg) kg 0,45
Substitution of primary metals with net scrap
kg 0,023
from PWB, with components (kg)
Substitution of copper with net scrap from PWB,
kg 0,035
without components (kg)
7 / 14
LCA: Results
The LCA results are presented below for the declared unit defined on page 2 of the EPD document.
Environmental impact
Indicator Unit A1 A2 A3 A4 A5
GWP-total kg CO2 -eq 8,50E+01 3,02E-01 3,67E+00 8,65E-01 3,43E-01
GWP-fossil kg CO2 -eq 8,45E+01 3,01E-01 3,45E+00 8,65E-01 3,24E-03
GWP-biogenic kg CO2 -eq 3,96E-01 1,19E-04 2,06E-01 3,58E-04 3,40E-01
GWP-luluc kg CO2 -eq 1,24E-01 1,22E-04 1,18E-02 3,08E-04 1,07E-06
ODP kg CFC11 -eq 6,57E-06 6,77E-08 1,92E-07 1,96E-07 6,83E-10
AP mol H+ -eq 6,31E-01 2,15E-03 1,31E-02 2,48E-03 1,53E-05
EP-FreshWater kg P -eq 1,16E-02 2,24E-06 2,39E-04 6,91E-06 2,66E-08
EP-Marine kg N -eq 9,08E-02 4,94E-04 2,63E-03 4,92E-04 5,07E-06
EP-Terrestial mol N -eq 1,01E+00 5,50E-03 3,44E-02 5,50E-03 5,49E-05
POCP kg NMVOC -eq 3,38E-01 1,63E-03 7,99E-03 2,11E-03 1,58E-05
ADP-minerals&metals1 kg Sb-eq 1,06E-02 7,45E-06 2,63E-05 2,39E-05 7,87E-08
ADP-fossil1 MJ 1,09E+03 4,46E+00 4,57E+01 1,31E+01 4,53E-02
WDP1 m3 3,97E+03 3,88E+00 5,38E+02 1,26E+01 5,74E-02
Indicator Unit B6 C1 C2 C3 C4 D
GWP-total kg CO2 -eq 1,65E+02 0,00E+00 2,88E-01 1,64E+00 1,29E-01 -2,20E+00
GWP-fossil kg CO2 -eq 1,60E+02 0,00E+00 2,88E-01 1,64E+00 1,29E-01 -2,19E+00
GWP-biogenic kg CO2 -eq 4,42E+00 0,00E+00 1,19E-04 1,54E-03 5,49E-05 -5,51E-03
GWP-luluc kg CO2 -eq 6,60E-01 0,00E+00 1,03E-04 5,16E-04 4,43E-04 -4,46E-03
ODP kg CFC11 -eq 1,10E-05 0,00E+00 6,53E-08 6,66E-08 8,16E-09 -4,20E-03
AP mol H+ -eq 1,25E+00 0,00E+00 8,28E-04 1,48E-03 3,96E-04 -1,30E-01
EP-FreshWater kg P -eq 1,15E-02 0,00E+00 2,30E-06 1,66E-05 2,65E-06 -8,06E-04
EP-Marine kg N -eq 1,37E-01 0,00E+00 1,64E-04 3,52E-04 1,53E-04 -6,77E-03
EP-Terrestial mol N -eq 1,79E+00 0,00E+00 1,83E-03 3,86E-03 1,13E-03 -9,39E-02
POCP kg NMVOC -eq 4,81E-01 0,00E+00 7,02E-04 1,04E-03 4,32E-04 -2,73E-02
ADP-minerals&metals1 kg Sb-eq 1,19E-02 0,00E+00 7,96E-06 2,70E-06 4,42E-07 -2,26E-03
ADP-fossil1 MJ 2,18E+03 0,00E+00 4,36E+00 3,56E+00 1,01E+00 -2,55E+01
WDP1 m3 3,80E+05 0,00E+00 4,22E+00 2,10E+01 1,08E+01 -1,66E+01
GWP-total = Global Warming Potential total; GWP-fossil = Global Warming Potential fossil fuels; GWP-biogenic = Global Warming Potential biogenic; GWP-luluc =
Global Warming Potential land use and land use change; ODP = Depletion potential of the stratospheric ozone layer; AP = Acidification potential, Accumulated
Exceedance; EP-freshwater = Eutrophication potential, fraction of nutrients reaching freshwater end compartment: EP-marine = Eutrophication potential, fraction of
nutrients reaching marine end compartment; EP-terrestrial = Eutrophication potential, Accumulated Exceedance; POCP = Formation potential of tropospheric ozone;
ADP-minerals&metals = Abiotic depletion potential for non-fossil resources; ADP-fossil = Abiotic depletion for fossil resources potential; WDP = Water (user)
deprivation potential, deprivation-weighted water consumption
"Reading example: 9,0 E-03 = 9,0*10-3 = 0,009"
*INA Indicator Not Assessed
1. The results of this environmental impact indicator shall be used with care as the uncertainties on these results are high or as there is limited experienced with the
indicator
Remarks to environmental impacts
8 / 14
The product is compliant with the European RoHS Directive 2011/65/EU on Restriction of the use of certain Hazardous Substances in Electrical and
Electronic equipment and with the European REACH regulation (EC) No 1907/2006 on Registration, Evaluation, Authorization and Restriction of
Chemicals.
9 / 14
Additional environmental impact indicators
Indicator Unit A1 A2 A3 A4 A5
PM Disease incidence 4,61E-06 1,58E-08 1,76E-07 5,29E-08 2,26E-10
IRP2 kgBq U235 -eq 4,18E+00 1,94E-02 1,93E-01 5,71E-02 1,94E-04
ETP-fw1 CTUe 4,89E+03 3,21E+00 8,01E+01 9,69E+00 6,04E-02
HTP-c1 CTUh 2,16E-07 0,00E+00 1,59E-09 0,00E+00 2,00E-12
HTP-nc1 CTUh 5,16E-06 3,16E-09 5,86E-08 1,06E-08 7,60E-11
SQP1 dimensionless 3,15E+02 2,80E+00 8,00E+01 9,14E+00 3,04E-02
Indicator Unit B6 C1 C2 C3 C4 D
PM Disease incidence 8,96E-06 0,00E+00 1,76E-08 1,58E-08 6,77E-09 -3,24E-07
IRP2 kgBq U235 -eq 3,96E+01 0,00E+00 1,90E-02 1,68E-02 3,65E-03 -7,47E-02
ETP-fw1 CTUe 9,94E+03 0,00E+00 3,23E+00 1,45E+01 5,31E+02 -1,03E+03
HTP-c1 CTUh 4,75E-07 0,00E+00 0,00E+00 2,34E-09 2,59E-10 -1,08E-08
HTP-nc1 CTUh 1,12E-05 0,00E+00 3,53E-09 1,13E-07 2,53E-09 -6,17E-07
SQP1 dimensionless 1,10E+03 0,00E+00 3,05E+00 1,14E+00 2,48E+00 -2,39E+01
PM = Particulate Matter emissions; IRP = Ionizing radiation – human health; ETP-fw = Eco toxicity – freshwater; HTP-c = Human toxicity – cancer effects; HTP-nc =
Human toxicity – non cancer effects; SQP = Potential Soil Quality Index (dimensionless)
"Reading example: 9,0 E-03 = 9,0*10-3 = 0,009"
*INA Indicator Not Assessed
1. The results of this environmental impact indicator shall be used with care as the uncertainties on these results are high or as there is limited experienced with the
indicator
2. This impact category deals mainly with the eventual impact of low dose ionizing radiation on human health of the nuclear fuel cycle. It does not consider effects due
to possible nuclear accidents, occupational exposure nor due to radioactive waste disposal in underground facilities. Potential ionizing radiation from the soil, from
radon and from some construction materials is also not measured by this indicator.
10 / 14
Resource use
Indicator Unit A1 A2 A3 A4 A5
PERE MJ 1,07E+02 5,96E-02 4,76E+01 1,87E-01 7,45E-04
PERM MJ 1,64E+00 0,00E+00 0,00E+00 0,00E+00 -1,64E+00
PERT MJ 1,09E+02 5,96E-02 4,76E+01 1,87E-01 -1,64E+00
PENRE MJ 1,07E+03 4,46E+00 4,57E+01 1,31E+01 4,53E-02
PENRM MJ 2,73E+01 0,00E+00 0,00E+00 0,00E+00 0,00E+00
PENRT MJ 1,09E+03 4,46E+00 6,05E+01 1,31E+01 4,53E-02
SM kg 5,55E+00 0,00E+00 3,12E-02 0,00E+00 4,59E-05
RSF MJ 2,22E+00 2,09E-03 1,11E+00 6,70E-03 2,47E-05
NRSF MJ 1,12E+01 8,41E-03 1,26E+00 2,39E-02 1,02E-04
FW m3 8,99E-01 4,46E-04 1,21E-01 1,40E-03 2,14E-05
Indicator Unit B6 C1 C2 C3 C4 D
PERE MJ 2,83E+04 0,00E+00 6,24E-02 6,00E-01 2,45E-01 -8,06E+00
PERM MJ 0,00E+00 0,00E+00 0,00E+00 0,00E+00 0,00E+00 0,00E+00
PERT MJ 2,83E+04 0,00E+00 6,24E-02 6,00E-01 2,45E-01 -8,06E+00
PENRE MJ 2,19E+03 0,00E+00 4,36E+00 3,56E+00 1,01E+00 -2,55E+01
PENRM MJ 0,00E+00 0,00E+00 0,00E+00 -2,93E+01 0,00E+00 0,00E+00
PENRT MJ 2,19E+03 0,00E+00 4,36E+00 -2,57E+01 1,01E+00 -2,90E+01
SM kg 0,00E+00 0,00E+00 0,00E+00 1,20E-03 9,46E-03 2,78E-01
RSF MJ 2,22E+01 0,00E+00 2,23E-03 1,17E-02 1,51E-03 2,10E-02
NRSF MJ 5,53E+01 0,00E+00 7,98E-03 -2,79E-03 4,49E-02 2,35E-01
FW m3 2,11E+02 0,00E+00 4,66E-04 4,17E-03 9,37E-04 -2,65E-02
PERE = Use of renewable primary energy excluding renewable primary energy resources used as raw materials; PERM = Use of renewable primary energy resources used
as raw materials; PERT = Total use of renewable primary energy resources; PENRE = Use of non renewable primary energy excluding non-renewable primary energy
resources used as raw materials; PENRM = Use of non renewable primary energy resources used as raw materials; PENRT = Total use of non renewable primary energy
resources; SM = Use of secondary materials; RSF = Use of renewable secondary fuels; NRSF = Use of non-renewable secondary fuels; FW = Net use of fresh water
"Reading example: 9,0 E-03 = 9,0*10-3 = 0,009"
*INA Indicator Not Assessed
11 / 14
End of life - Waste
Indicator Unit A1 A2 A3 A4 A5
HWD kg 5,07E-01 2,25E-04 3,12E-02 6,74E-04 2,00E-04
NHWD kg 1,57E+01 1,91E-01 3,41E-01 6,36E-01 2,26E-03
RWD kg 3,38E-03 3,04E-05 1,34E-04 8,91E-05 2,99E-07
Indicator Unit B6 C1 C2 C3 C4 D
HWD kg 1,40E+00 0,00E+00 2,25E-04 8,68E-04 2,64E-01 -1,04E-02
NHWD kg 1,68E+02 0,00E+00 2,12E-01 1,35E-01 1,35E+00 -5,75E-01
RWD kg 1,95E-02 0,00E+00 2,97E-05 1,79E-05 4,07E-06 -6,46E-05
HWD = Hazardous waste disposed; NHWD = Non-hazardous waste disposed; RWD = Radioactive waste disposed
"Reading example: 9,0 E-03 = 9,0*10-3 = 0,009"
*INA Indicator Not Assessed
End of life - Output flow
Indicator Unit A1 A2 A3 A4 A5
CRU kg 0,00E+00 0,00E+00 0,00E+00 0,00E+00 0,00E+00
MFR kg 1,23E-02 0,00E+00 3,51E+00 0,00E+00 1,86E-01
MER kg 1,06E-03 0,00E+00 1,10E-02 0,00E+00 2,72E-07
EEE MJ 3,10E-03 0,00E+00 1,06E-01 0,00E+00 1,14E-02
EET MJ 4,70E-02 0,00E+00 1,61E+00 0,00E+00 1,73E-01
Indicator Unit B6 C1 C2 C3 C4 D
CRU kg 0,00E+00 0,00E+00 0,00E+00 0,00E+00 0,00E+00 0,00E+00
MFR kg 0,00E+00 0,00E+00 0,00E+00 3,29E+00 5,00E-03 2,37E-01
MER kg 0,00E+00 0,00E+00 0,00E+00 1,07E-04 1,17E-04 -5,20E-05
EEE MJ 0,00E+00 0,00E+00 0,00E+00 6,57E-01 1,10E-03 -6,71E-04
EET MJ 0,00E+00 0,00E+00 0,00E+00 9,94E+00 1,67E-02 -1,02E-02
CRU = Components for re-use; MFR = Materials for recycling; MER = Materials for energy recovery; EEE = Exported energy electrical; EET = Exported energy thermal
"Reading example: 9,0 E-03 = 9,0*10-3 = 0,009"
*INA Indicator Not Assessed
Biogenic Carbon Content
Indicator Unit At the factory gate
Biogenic carbon content in product kg C 0,00E+00
Biogenic carbon content in accompanying packaging kg C 9,26E-02
Note: 1 kg biogenic carbon is equivalent to 44/12 kg CO2
12 / 14
Additional requirements
Greenhouse gas emissions from the use of electricity in the manufacturing phase
National production mix from import, low voltage (production of transmission lines, in addition to direct emissions and losses in grid) of applied
electricity for the manufacturing process (A3).
Electricity mix Source Amount Unit
Electricity, Denmark (kWh) ecoinvent 3.6 338,20 g CO2-eq/kWh
Dangerous substances
The product contains substances given by the REACH Candidate list that are less than 0,1 % by weight.
Name CASNo Amount
Lead 7439-92-1 <0,1%
Indoor environment
No effect on indoor environment.
Additional Environmental Information
Additional environmental impact indicators required in NPCR Part A for construction products
Indicator Unit A1 A2 A3 A4 A5
GWPIOBC kg CO2 -eq 8,39E+01 3,02E-01 4,38E+00 8,65E-01 0,00E+00
Indicator Unit B6 C1 C2 C3 C4 D
GWPIOBC kg CO2 -eq 1,65E+02 0,00E+00 2,88E-01 1,64E+00 3,45E-02 -2,38E+00
GWP-IOBC: Global warming potential calculated according to the principle of instantaneous oxidation. In order to increase the transparency of biogenic carbon​
contribution to climate impact, the indicator GWP-IOBC is required as it declares climate impacts calculated according to the principle of instantaneous oxidation.​
GWP-IOBC is also referred to as GWP-GHG in context to Swedish public procurement legislation.
13 / 14
Bibliography
ISO 14025:2010. Environmental labels and declarations - Type III environmental declarations - Principles and procedures. International
Organization for Standardization.
ISO 14044:2006. Environmental management - Life cycle assessment - Requirements and guidelines. International Organization for
Standardization.
EN 15804:2012+A2:2019. Environmental product declaration - Core rules for the product category of construction products. European
Committee for Standardization.
ISO 21930:2017. Sustainability in buildings and civil engineering works - Core rules for environmental product declarations of construction
products. International Organization for Standardization.
EN 50693:2019. Product category rules for life cycle assessments of electronic and electrical products and systems. European Committee for
Standardization.
Ecoinvent v3, 2019. Allocation, cut-off by classification. Swiss Centre of Life Cycle Inventories.
Iversen et al., (2021). eEPD v2021.09, background information for EPD generator tool system verification, LCA.no. Report number: 07.21. System
verification report.
Philis et al., (2022). EPD generator for IBU PCR part B for luminaires, lamps, and components for luminaires, background information for EPD
generator application and LCA data, LCA.no. Report number: 04.22. PCR verification report.
EPD Norway (2022). NPCR Part A: Construction products and services. The Norwegian EPD foundation. Version 2.0 published 24.03.2021.
IBU (2017). PCR part B for luminaires, lampes and components for luminaires. Institut Bauen und Umwelt e.V. Version 1.7, published 30.11.2017.
Program operator and publisher Phone: +47 977 22 020
The Norwegian EPD Foundation e-mail: post@epd-norge.no
Post Box 5250 Majorstuen, 0303 Oslo, Norway web: www.epd-norge.no
Owner of the declaration: Phone: +47 90021243
SG Armaturen AS e-mail: audun.skare@sg-as.no
Skytterheia 25, 4790 Lillesand, Norway web: www.sg-as.com
Author of the Life Cycle Assessment Phone: +47 916 50 916
LCA.no AS e-mail: post@lca.no
Dokka 6A, 1671 Kråkerøy, Norway web: www.lca.no
Developer of EPD generator Phone: +47 916 50 916
LCA.no AS e-mail: post@lca.no
Dokka 6A, 1671 Kråkerøy, Norway web: www.lca.no
ECO Platform web: www.eco-platform.org
ECO Portal web: ECO Portal
14 / 14
