ENVIRONMENTAL PRODUCT DECLARATION
as per ISO 14025 and EN 15804+A2
Owner of the Declaration VIR – Valvoindustria Ing. Rizzio S.p.A.
Publisher Institut Bauen und Umwelt e.V. (IBU)
Programme holder Institut Bauen und Umwelt e.V. (IBU)
Declaration number EPD-VIR-20230495-IBC1-EN
Issue date 11/01/2024
Valid to 10/01/2029
Different bronze valves family constituted by full bore ball valves,
gate valves and fixed-orifice balancing valves
Vir Valvoindustria Ing. Rizzio Spa
www.ibu-epd.com | https://epd-online.com
1. General Information
Vir Valvoindustria Ing. Rizzio Spa Different bronze valves family constituted by full
bore ball valves, gate valves and fixed-orifice
balancing valves
Programme holder Owner of the declaration
IBU – Institut Bauen und Umwelt e.V. VIR – Valvoindustria Ing. Rizzio S.p.A.
Hegelplatz 1 Via circonvallazione 10
10117 Berlin 13018 Valduggia (VC)
Germany Italy
Declaration number Declared product / declared unit
EPD-VIR-20230495-IBC1-EN The declared unit is 1 kg of the average valve of the family
This declaration is based on the product category rules: Scope:
Fittings and connections for water supply, 01/08/2021 This Environmental Product Declaration refers to a declared unit of 1 kg of
(PCR checked and approved by the SVR) the average valve of the bronze family - type '380' '100/100LK' and 'Serie
9580' - produced at the production site of VIR - Valvoindustria Ing. Rizzio
S.p.A. in Via circonvallazione 10, 13018 Valduggia (VC), Italy.
Issue date The owner of the declaration shall be liable for the underlying information
and evidence; the IBU shall not be liable with respect to manufacturer
11/01/2024
information, life cycle assessment data and evidences.
The EPD was created according to the specifications of EN 15804+A2. In
Valid to
the following, the standard will be simplified as EN 15804.
10/01/2029
Verification
The standard EN 15804 serves as the core PCR
Independent verification of the declaration and data according to ISO
14025:2011
internally X externally
Dipl.-Ing. Hans Peters
(Chairman of Institut Bauen und Umwelt e.V.)
Florian Pronold Vito D'Incognito,
(Managing Director Institut Bauen und Umwelt e.V.) (Independent verifier)
Environmental Product Declaration - Vir Valvoindustria Ing. Rizzio Spa - Different bronze valves family constituted by full bore ball valves, gate valves and fixed-orifice
1 balancing valves
2. Product
Name Value Unit
2.1 Product description/Product definition
Bronze 0.6455 kg
Brass 0.2396 kg
The process starts with the manufacturing of raw bronze pieces
for valves obtained from casting and hot-moulding then the Steel 0.0533 kg
pieces are mechanically worked and assembled with valves Aluminium 0.0158 kg
components (e.g. handles, gaskets, balls, fittings, etc.). ABS 0.0277 kg
Declared units refer to three different types of valves - 380,
PTFE 0.0092 kg
100/100LK and Serie 9580. Every valve typology contains
Polypropylene 0.0031 kg
valves with different dimensions and weights. However, the
same manufacturing process and the similarities of valves allow Polyoxymethylene 0.0023 kg
a declared unit based on a mass unit of products. EPDM rubber 0.0023 kg
NBR rubber 0.0008 kg
Graphite 0.0004 kg
This product contains substances listed in the candidate list
(date: 14.06.2023) exceeding 0.1 percentage by mass:
• Lead (CAS 7439-92-1) - concentration range: 1.6% -
2.8%.
2.6 Manufacture
For the use and application of the product, the respective
national provisions at the place of use apply, in Germany for
example the building codes of the federal states and the
corresponding national specifications.
2.2 Application
Model 380: Water and air from -10°C to 185°C
Model 100/100LK: Water from -10°C to 170°C
Model 9580: Water from -10°C to 130°C
2.3 Technical Data
The valves are tested according to EN 12266-1 standard.
Technical data
Name Value Unit
medium Water, air
Nominal diameter (DN) 10 - 80
Weight 0.000132 - 0.0062 t
Housing material Bronze
spindle material Bronze
Performance data of the product with respect to its
characteristics are in accordance with the relevant technical
provision.
2.4 Delivery status
The valves are delivered fully assembled, tested, and packaged
with a plastic envelope and a carton box, to Italy and to the rest
of the world (mainly where manufacturer's branches are
located). For land transport the products are delivered by
trucks, while for sea routes they are transported by cargo ships.
2.7 Environment and health during manufacturing
2.5 Base materials/Ancillary materials The manufacturing stage is made in accordance with the Italian
regulation.
2.8 Product processing/Installation
1. FOUNDRY: preparation of cores and shells, material
preparation, bronze casting, stamping, cooling and
valve removal, finishing;
2. BLASTING: the bronze valves are subjected to a
surface treatment by a sandblasting machine and steel
grit;
3. TURNING: the valves are machined by transfer
machines or numerical control machining centres (CNC)
Environmental Product Declaration - Vir Valvoindustria Ing. Rizzio Spa - Different bronze valves family constituted by full bore ball valves, gate valves and fixed-orifice
2 balancing valves
cooled by cooling oil. The brass turning is dried by
centrifuge and conveyed to a silo for sale as a 2.13 Extraordinary effects
secondary raw material; Fire
4. ASSEMBLY: the valves are assembled by automatic Due to the predominant use of bronze and brass which are
machines by performing 100% air test and fixing the considered nonflammable or flame retardant, no additional
components with adhesives; influence on the environment in case of fire is to be expected.
5. PACKAGING AND STORAGE: following the quality Water
check, the valves are packaged ensuring adequate Two water contaminants can be found into the valve: lead and
protection and stored for shipment. nickel.
2.9 Packaging Mechanical destruction
The packaging materials are the following: No impacts on the environment are expected in the case of an
unforeseeable mechanical destruction.
• Wood (11.1 %);
• Paper and cardboard (87.5 %);
2.14 Re-use phase
• Polyethylene (1.3 %);
With reference to the material composition of the product
• Plastic film (0.1 %).
system in accordance with section 2.5, the metallurgical
The disposal of the packaging is consistent with the regulation
materials contained in the product are suitable for material
of the countries of sale.
recycling.
2.10 Condition of use
2.15 Disposal
No auxiliaries or consumables are incurred during
If there is no specific regulation for the valve disposal, VIR
maintenance, and use of the Valves. Regular maintenance is
reccommends to:
advised to ensure a service life of at least 10 years.
- Recycle the metal parts to reuse it as raw material;
2.11 Environment and health during use - Send to specifical end-of-life guarantees and others PTFE
(Polytetrafluoroethylene), NBR (Nitril-Butadiene-rubber) and
There are no known impact relations between product,
EPDM (ethylene propylene diene monomer rubber) elements,
environment and health during use.
since they could be contaminated by the liquids flowing in the
2.12 Reference service life valve;
Regular maintenance is advised to ensure a service life which - Collect all the packaging to the local waste sorting system.
is minimum 10 years.
2.16 Further information
Contact data for more detailed information: Please refer to the
last page of this Declaration
3. LCA: Calculation rules
Modules C1-C4
3.1 Declared Unit The modules include the environmental impacts for dismantling
The functional unit is constituted as the weighted average of the valve and the treatment of the waste categories until end-
between the three types of valves. The mass of assembled of-waste status (EoW) is reached, including the associated
products corresponding to each family has been used as the transports at the end of the product life cycle.
weight of the average.
Deklarierte Einheit
Module D
Name Value Unit
Identification of the benefits and impacts of the product outside
Declared unit 1 kg
the system boundary. Recycling of metal scrap results in credits
Gross Density 8700 kg/m3 of the raw material.
The use of an average EPD seems to be consistent due to the
3.3 Estimates and assumptions
low variability of the three types of valves. All the valves
The bronze used in the valves production was modelled
included in the average are manufactured by the same
assuming that it comes only from new material. In C2, the
producer, in the same plant, with the same manufacturing
distance between the use site and the disposal site is assumed
proccess. Since there is only one production site the
to be 50 km.
modellization is highly geographically representative and
background data have the same inluence on all the considered 3.4 Cut-off criteria
types of valves.
The effect associated with the neglected mass shares is less
than 5 % of the effect categories per module.
3.2 System boundary
Type of the EPD: cradle to gate with options 3.5 Background data
The LCA software Simapro 9.5.0.1 was used to model the life
Modules A1-A3, A4 and A5
cycle. The entire manufacturing process, as well as energy
Here there is the production of the necessary raw materials and
consumption, were modelled on the basis of manufacturer
energies, including all corresponding upstream chains and the
specific data. However, generic background datasets were
actual procurement transports. Furthermore, the entire
used for the upstream and downstream processes. The
manufacturing phase was mapped, including the treatment of
background datasets used were taken from the current version
production waste until the endofwaste status (EoW) was
of the Ecoinvent 3.9.1 database.
reached. In addition the distribution transports (A4) and the
Where possible, Italian datasets were used for modules A1-A3,
installation (with also packaging waste generated during
A5, C1, C3, C4 and D; the corresponding European datasets
installation) was taken into account.
for distribution transports (A4, C2).
Environmental Product Declaration - Vir Valvoindustria Ing. Rizzio Spa - Different bronze valves family constituted by full bore ball valves, gate valves and fixed-orifice
3 balancing valves
lifespan: Global
3.6 Data quality
The background datasets used for accounting purposes mainly
originate from the respective updated Ecoinvent 3.9.1 3.9 Allocation
databases, through the software Simapro 9.5.0.1, at the time of All raw materials, and supplies could be (clearly) assigned to
calculation. The data for the examined products was captured the declared product. All required energies, waste produced in
on the basis of evaluations of internal production and the manufacturing processes and production emissions are
environmental data, the collection of LCA relevant data within allocated to each family on the basis of the total mass of valves
the supply chain, as well as the evaluation of relevant data for produced. No byproducts are produced or any other allocation
the energy supply. The collected data were checked for is needed.
plausibility and consistency. Good representativity can be
3.10 Comparability
assumed.
Basically, a comparison or an evaluation of EPD data is only
3.7 Period under review possible if all the data sets to be compared were created
Life cycle assessment data refer to 2021. according to EN 15804 and the building context, respectively
the product-specific characteristics of performance, are taken
3.8 Geographic Representativeness into account. The background database used is Ecoinvent
Land or region, in which the declared product system is 3.9.1, through the software Simapro 9.5.0.1.
manufactured, used or handled at the end of the product´s
4. LCA: Scenarios and additional technical information
Characteristic product properties of biogenic carbon The A1-A3, C1, C2, C3, C4 and D stage have been considered
There is no biogenic carbon content in the product, while separately. The optional A4 and A5 stage have also been
differently, the packaging has a non-zero amount. considered.
Transport from the gate to the site (A4)
Note: 1 kg of biogenic carbon is equivalent to 44/12 kg of CO .
2
Name Value Unit
Information on describing the biogenic carbon content at
Land transport distance 255.57 km
factory gate
Sea transport distance 5932.27 km
Name Value Unit
Regular maintenance is advised to ensure a service life of at
kg
Biogenic carbon content in product - least 10 years.
C
Biogenic carbon content in accompanying kg
0.13301
packaging C
Environmental Product Declaration - Vir Valvoindustria Ing. Rizzio Spa - Different bronze valves family constituted by full bore ball valves, gate valves and fixed-orifice
4 balancing valves
5. LCA: Results
The following table shows the results of the LCA for 1kg of Bronze Valve of the VIR models: 380, 100/100 LK and Serie 9580.
DESCRIPTION OF THE SYSTEM BOUNDARY (X = INCLUDED IN LCA; MND = MODULE OR INDICATOR NOT DECLARED; MNR
= MODULE NOT RELEVANT)
Benefits and
Construction loads beyond
Product stage Use stage End of life stage
process stage the system
boundaries
la ire ta m w a Ry lp p u s tro p s n a rT g n iru tc a fu n a M e h t m o rf tro p s n a rTe tis e h t o t e ta g y lb m e s s A e s U e c n a n e tn ia M ria p e R tn e m e c a lp e R tn e m h s ib ru fe R y g re n e la n o ita re p Oe s u re ta w la n o ita re p Oe s u n o itc u rts n o c -e Dn o itilo m e d tro p s n a rT g n is s e c o rp e ts a W la s o p s iD -e s u e R-y re v o c e R-g n ilc y c e Rla itn e to p
A1 A2 A3 A4 A5 B1 B2 B3 B4 B5 B6 B7 C1 C2 C3 C4 D
X X X X X MND MND MNR MNR MNR MND MND X X X X X
RESULTS OF THE LCA - ENVIRONMENTAL IMPACT according to EN 15804+A2: 1 kg Average Bronze Valve
Parameter Unit A1-A3 A4 A5 C1 C2 C3 C4 D
GWP-total kg CO 2 eq 1.31E+01 1.08E-01 3.12E-02 0 9.43E-03 9.86E-02 4.97E-03 -4.09E+00
GWP-fossil kg CO 2 eq 1.31E+01 1.08E-01 7.3E-03 0 9.42E-03 5.72E-02 4.97E-03 -4.07E+00
GWP-biogenic kg CO 2 eq 7.09E-02 7.63E-05 -8.58E-03 3.1E-05 2.39E-02 0 8.51E-06 4.13E-02
GWP-luluc kg CO 2 eq 2.04E-02 4.14E-05 9.8E-03 6.99E-05 3.09E-07 0 4.57E-06 1.43E-04
ODP kg CFC11 eq 3.27E-05 1.96E-09 1.74E-11 0 2.05E-10 7.52E-10 1.38E-11 -4.55E-08
AP mol H+ eq 4.86E-01 1.95E-03 5.61E-06 0 3.07E-05 3.93E-04 4.44E-06 -3.13E-01
EP-freshwater kg P eq 3.83E-02 5.37E-06 1.45E-07 0 6.59E-07 1.27E-05 8.73E-08 -2.51E-02
EP-marine kg N eq 2.82E-02 5.02E-04 1.47E-05 0 1.06E-05 1.55E-04 1.05E-04 -1.59E-02
EP-terrestrial mol N eq 3.84E-01 5.53E-03 2.49E-05 0 1.11E-04 1.38E-03 1.71E-05 -2.22E-01
kg NMVOC
POCP 1.1E-01 1.57E-03 8.3E-06 0 4.59E-05 4.39E-04 6.91E-06 -6.23E-02
eq
ADPE kg Sb eq 6.94E-03 2.13E-07 1.25E-09 0 3.02E-08 4.89E-07 1.33E-09 -4.77E-03
ADPF MJ 1.6E+02 1.42E+00 7.66E-03 0 1.33E-01 6.79E-01 1.28E-02 -4.99E+01
m3 world eq
WDP 7.95E+00 4.44E-03 4.46E-04 0 5.44E-04 5.46E-03 5.32E-04 -4.11E+00
deprived
GWP = Global warming potential; ODP = Depletion potential of the stratospheric ozone layer; AP = Acidification potential of land and water; EP =
Eutrophication potential; POCP = Formation potential of tropospheric ozone photochemical oxidants; ADPE = Abiotic depletion potential for non-fossil
resources; ADPF = Abiotic depletion potential for fossil resources; WDP = Water (user) deprivation potential)
RESULTS OF THE LCA - INDICATORS TO DESCRIBE RESOURCE USE according to EN 15804+A2: 1 kg Average Bronze Valve
Parameter Unit A1-A3 A4 A5 C1 C2 C3 C4 D
PERE MJ 1.68E+01 9.9E-03 1.3E-04 0 1.29E-03 1.31E-02 1.81E-04 -1.07E+01
PERM MJ 1.05E+01 5.96E-03 9.14E-05 0 7.85E-04 1.94E-02 8.69E-05 -2.98E+00
PERT MJ 2.73E+01 1.59E-02 2.21E-04 0 2.07E-03 3.25E-02 2.68E-04 -1.37E+01
PENRE MJ 1.59E+02 1.42E+00 -3.59E-02 0 1.33E-01 6.79E-01 1.28E-02 -4.99E+01
PENRM MJ 9.55E-01 0 4.36E-02 0 0 0 0 1.18E-02
PENRT MJ 1.6E+02 1.42E+00 7.66E-03 0 1.33E-01 6.79E-01 1.28E-02 -4.99E+01
SM kg ND ND ND ND ND ND ND ND
RSF MJ ND ND ND ND ND ND ND ND
NRSF MJ ND ND ND ND ND ND ND ND
FW m3 8.15E+00 4.44E-03 4.43E-04 0 5.42E-04 5.48E-03 5.32E-04 -4.27E+00
PERE = Use of renewable primary energy excluding renewable primary energy resources used as raw materials; PERM = Use of renewable primary
energy resources used as raw materials; PERT = Total use of renewable primary energy resources; PENRE = Use of non-renewable primary energy
excluding non-renewable primary energy resources used as raw materials; PENRM = Use of non-renewable primary energy resources used as raw
materials; PENRT = Total use of non-renewable primary energy resources; SM = Use of secondary material; RSF = Use of renewable secondary fuels;
NRSF = Use of non-renewable secondary fuels; FW = Use of net fresh water
RESULTS OF THE LCA – WASTE CATEGORIES AND OUTPUT FLOWS according to EN 15804+A2:
1 kg Average Bronze Valve
Parameter Unit A1-A3 A4 A5 C1 C2 C3 C4 D
HWD kg 1.55E-03 8E-06 3.85E-08 0 8.5E-07 3.9E-06 6.26E-08 -1.74E-04
NHWD kg 2.99E+00 3.52E-02 1.72E-02 0 6.52E-03 3.27E-02 4.91E-02 -1.69E+00
RWD kg 3.03E-04 3.02E-07 3.44E-09 0 4.34E-08 3.66E-07 4.89E-09 -1.12E-04
CRU kg 0 0 0 0 0 0 0 0
MFR kg 0 0 0 0 0 6.46E-01 0 0
MER kg 0 0 5.38E-03 0 0 0 0 0
EEE MJ 0 0 0 0 0 0 0 0
EET MJ 0 0 0 0 0 0 0 0
Environmental Product Declaration - Vir Valvoindustria Ing. Rizzio Spa - Different bronze valves family constituted by full bore ball valves, gate valves and fixed-orifice
5 balancing valves
HWD = Hazardous waste disposed; NHWD = Non-hazardous waste disposed; RWD = Radioactive waste disposed; CRU = Components for re-use;
MFR = Materials for recycling; MER = Materials for energy recovery; EEE = Exported electrical energy; EET = Exported thermal energy
RESULTS OF THE LCA – additional impact categories according to EN 15804+A2-optional:
1 kg Average Bronze Valve
Parameter Unit A1-A3 A4 A5 C1 C2 C3 C4 D
Disease
PM ND ND ND ND ND ND ND ND
incidence
IR kBq U235 eq ND ND ND ND ND ND ND ND
ETP-fw CTUe ND ND ND ND ND ND ND ND
HTP-c CTUh ND ND ND ND ND ND ND ND
HTP-nc CTUh ND ND ND ND ND ND ND ND
SQP SQP ND ND ND ND ND ND ND ND
PM = Potential incidence of disease due to PM emissions; IR = Potential Human exposure efficiency relative to U235; ETP-fw = Potential comparative
Toxic Unit for ecosystems; HTP-c = Potential comparative Toxic Unit for humans (cancerogenic); HTP-nc = Potential comparative Toxic Unit for humans
(not cancerogenic); SQP = Potential soil quality index
Disclaimer 1 – for the indicator “Potential Human exposure efficiency relative to U235”. This impact category deals mainly with the
eventual impact of low-dose ionizing radiation on human health of the nuclear fuel cycle. It does not consider effects due to possible
nuclear accidents, occupational exposure or radioactive waste disposal in underground facilities. Potential ionizing radiation from the
soil, radon and from some construction materials is also not measured by this indicator.
Disclaimer 2 – for the indicators “abiotic depletion potential for non-fossil resources”, “abiotic depletion potential for fossil resources”,
“water (user) deprivation potential, deprivation-weighted water consumption”, “potential comparative toxic unit for ecosystems”,
“potential comparative toxic unit for humans – cancerogenic”, “Potential comparative toxic unit for humans - not cancerogenic”,
“potential soil quality index”. The results of this environmental impact indicator shall be used with care as the uncertainties on these
results are high as there is limited experience with the indicator.
6. LCA: Interpretation
of-life (C1-C4) stages results show to have low relevance.
Specifically, the main impacts are in the A1 and A3 modules
The EN 15804 characterization factors were used for the and they are generated by the material production, while the
evaluation. The results of the EN 15804 categories refer to the transport related modules impacts are very low (A2 and A4).
potential environmental impacts over a period of 100 years.The The negative value related to GWP - Biogenic refers to the
main impacts clearly come from A1 - A3 stages while the end- presence of wood in the packaging.
7. Requisite evidence
Environmental Product Declaration - Vir Valvoindustria Ing. Rizzio Spa - Different bronze valves family constituted by full bore ball valves, gate valves and fixed-orifice
6 balancing valves
8. References
Standards procedures.
EN 15804 Further References
EN 15804:2012+A1 2013, Sustainability of construction works
— Environmental Product Declarations — Core rules for the SimaPro
product category of construction products. SimaPro software and databases. Version 9.4.0.2, PRè
Sustainability B.V. https://simapro.com/, 2023.
EN 15804
EN 15804:2012+A2:2019+AC:2021, Sustainability of Ecoinvent Version 3.8
construction works — Environmental Product Declarations — Database for life cycle assessment (life cycle inventory data),
Core rules for the product category of construction products. Version 3.8, 2021.
EN 12266-1 Product Category Rules Part A
EN 12266-1:2012, Industrial valves - Testing of metallic valves - Calculation Rules for the Life Cycle Assessment and
Part 1: Pressure tests, test procedures and acceptance Requirements on the Project Report. Version 2.1 (17.11.2021).
criteria - Mandatory requirements.
Product Category Rules Part B
ISO 14025 Requirements on the EPD for Fittings and connections for
EN ISO 14025:2011, Environmental labels and declarations — water supply. Version 5 (31.05.2023).
Type III environmental declarations — Principles and
Environmental Product Declaration - Vir Valvoindustria Ing. Rizzio Spa - Different bronze valves family constituted by full bore ball valves, gate valves and fixed-orifice
7 balancing valves
Publisher
Institut Bauen und Umwelt e.V. +49 (0)30 3087748- 0
Hegelplatz 1 info@ibu-epd.com
10117 Berlin www.ibu-epd.com
Germany
Programme holder
Institut Bauen und Umwelt e.V. +49 (0)30 3087748- 0
Hegelplatz 1 info@ibu-epd.com
10117 Berlin www.ibu-epd.com
Germany
Author of the Life Cycle Assessment
ICIM Consulting srl +39 02 72534800
Piazza Don Enrico Mapelli 75 info@icimconsulting.it
20099 Sesto San Giovanni www.icimconsulting.it
Italy
Owner of the Declaration
VIR – Valvoindustria Ing. Rizzio S.p.A. +39016347891
Via circonvallazione 10 info@vironline.com
13018 Valduggia (VC) www.vironline.com
Italy
Environmental Product Declaration - Vir Valvoindustria Ing. Rizzio Spa - Different bronze valves family constituted by full bore ball valves, gate valves and fixed-orifice
8 balancing valves
