ENVIRONMENTAL PRODUCT DECLARATION
as per ISO 14025 and EN 15804+A2
Owner of the Declaration Astron Buildings S.A
Publisher Institut Bauen und Umwelt e.V. (IBU)
Programme holder Institut Bauen und Umwelt e.V. (IBU)
Declaration number EPD-AST-20240033-IBI1-EN
Issue date 02.07.2024
Valid to 01.07.2029
Astron PLS Product (cold-formed steel elements made of
galvanized steel sheets)
Astron Buildings S.A.
www.ibu-epd.com | https://epd-online.com
1. General Information
Astron Buildings S.A. Astron PLS Product (cold-formed steel elements
made of galvanized steel sheets)
Programme holder Owner of the declaration
IBU – Institut Bauen und Umwelt e.V. Astron Buildings S.A
Hegelplatz 1 Route d’Ettelbruck 34
10117 Berlin 9230 Diekirch
Germany Luxembourg
Declaration number Declared product / declared unit
EPD-AST-20240033-IBI1-EN 1 t of PLS cold-formed steel elements made of galvanized steel sheets
This declaration is based on the product category rules: Scope:
Structural steels, 01.08.2021 The EPD represents 100% of cold-formed steel elements made of
(PCR checked and approved by the SVR) galvanized steel sheets produced by Astron Building S.A. in Diekirch.
The owner of the declaration shall be liable for the underlying information
and evidence; the IBU shall not be liable with respect to manufacturer
Issue date information, life cycle assessment data and evidences.
02.07.2024
The EPD was created according to the specifications of EN 15804+A2. In
the following, the standard will be simplified as EN 15804.
Valid to
Verification
01.07.2029
The standard EN 15804 serves as the core PCR
Independent verification of the declaration and data according to ISO
14025:2011
internally X externally
Dipl.-Ing. Hans Peters
(Chairman of Institut Bauen und Umwelt e.V.)
Florian Pronold Dr Naeem Adibi,
(Managing Director Institut Bauen und Umwelt e.V.) (Independent verifier)
1 Environmental Product Declaration - Astron Buildings S.A. - Astron PLS Product (cold-formed steel elements made of galvanized steel sheets)
2. Product
2.1 Product description/Product definition 2.4 Delivery status
This EPD applies to 1 t of PLS structural steel. PLS are The dimensions of the declared products may vary according to
structural steel elements which are made by roll forming or the intended application. The surface condition is galvanized.
bending thin steel plates to form structural sections with open
section forms (Zee, Cee, Sigma, Omega, L-angles, et cetera). 2.5 Base materials/Ancillary materials
The Astron PLS steel elements are of the steel grade S350GD Structural steels are non- or low-alloy steel products whose
Z275 or S390GD Z275 according to EN 10346. The raw carbon content is between 0 and 0.6 %. Iron is the main
material is galvanized and is on coils. component of steel sheets. The content of other alloy elements
For the placing on the market of the product in the European is significantly less. The exact chemical composition is defined
Union/European Free Trade Association (EU/EFTA) (with the for the S350 and S390 steel grades in the EN 10346. The
exception of Switzerland) Regulation (EU) No. 305/2011 (CPR) surfaces of PLS elements are covered by a zinc coating.
applies. The PRS elements need a declaration of performance
(DoP) taking into consideration EN 1090-1, Execution of steel 1) This product/article/at least one partial article contains
and aluminium structures Part 1: Requirements for conformity substances listed in the ECHA candidate list (date: 02.03.2022)
assessment of structural components and the CE-marking. exceeding 0.1 percentage by mass:
Alternatively, the DoP and CE marking are based on the ETA- • no
18/1027 'Astron Building System". 2) This product/article/at least one partial article contains other
carcinogenic, mutagenic, or toxic for reproduction (CMR)
For the application and use the respective national provisions substances in categories 1A or 1B which are not on the ECHA
apply. candidate list, exceeding 0.1 percentage by mass:
2.2 Application • no
Structural steel PLS elements are intended for bolted structures 3) Biocide products were added to this construction product or it
of industrial or other non-residential buildings. The PLS has been treated with biocide products (this then concerns a
elementsare fixed to the main structure ('primary structure') and treated product as defined by the (EU) Regulation on Biocidal
act as a substructurefor the building envelope. They are also Products No. 528/2012):
called 'secondary structures'. Examples are: • no
• single-storey buildings (industrial fabrication and/or
2.6 Manufacture
storage halls, exhibition halls, etc.)
The manufacturing follows the rules in EN 1090-4 Execution of
• multi-storey buildings (offices, shops, schools, car parks,
steel structures and aluminium structures – Part 4: Technical
etc.)
requirements for cold-formed structural steel elements and
• other industrial structures (power plants, sports or
cold-formed structures for roof, ceiling, floor and wall
leisure centers, convention centers, stations, etc.)
applications.
2.3 Technical Data
This EPD is valid for PLS steel elements of varied dimensions In the integrated PLS production line, the following steps are
and different forms of delivery. Specific information on executed:
dimension tolerances, constructional data as well as • uncoiling and straightening of the steel sheet
mechanical and chemical properties of the used steel can be • punching of holes
found in the relevant literature and/or the standards. PLS are • cutting to length by shearing
always produced from hot-dip galvanized steel of the quality • roll-forming (80% of volume) or break-pressing (20% of
Z275 or equivalent (for example ZA or ZM coatings). The volume) of the desired section
galvanization is performed according to EN ISO 1461 and with • bundling
mechanical stripping for zinc thickness control. Thickness Quality control: ISO 9001 monitoring according to the relevant
tolerances are the 'special tolerances' according to EN 10143. product standards, e.g. EN 1090 and ETA18-1027, including
Technical data of processed steel FPC auditing by a third party.
Name Value Unit 2.7 Environment and health during manufacturing
Density acc. EN 10025-1 7850 kg/m3 No measures relating to safety, health and environmental
Modulus of elasticity acc. EN 10025-1 210000 N/mm2 protection during the manufacturing process extending beyond
national guidelines are required.
Coefficient of thermal expansion acc. EN
12 10-6K-1
10025-1 2.8 Product processing/Installation
Thermal conductivity acc. EN 10025-1 48 W/(mK) Manufacturing/Erection:
Melting point acc. EN 10025-1 1536 °C Planning, manufacturing, erection and intended use of PLS
Shear modulus acc. EN 10025-1 81 kN/mm² elements have to be carried out depending on the respective
applications according to the generally recognized rules of
Performance data of the product in accordance with the
engineering and Astron erection recommendations.
declaration of performance with respect to its essential
The standard EN 1993-1-3 applies to the design of thin-walled
characteristics according to:
steel structures. It includes the requirements regarding
• EN 1090-1, Execution of steel and aluminium structures serviceability, bearing capacity, durability and fire resistance of
Part 1: Requirements for conformity assessment of steel structures (EC3). The Standard Parts 1+4 of EN 1090, or
structural components alternatively the ETA-18/1027 apply to the execution of
• ETA-18/1027 'Astron Building System secondary structures made of PLS steel elements and include
• EN ISO 1461, Hot dip galvanized coatings on fabricated the requirements for factory production control. In addition, the
iron and steel articles - Specifications and test methods European Standards will work in connection with national
2 Environmental Product Declaration - Astron Buildings S.A. - Astron PLS Product (cold-formed steel elements made of galvanized steel sheets)
amendments, national instructions, guidelines and publications,
Fire protection
as well as legal provisions.
Name Value
Regarding transport and storage of PLS elements, the
generally accepted requirements for securing loads have to be Building material class A1
observed. The material does not emit fumes or fire gases.
Occupational safety/Environmental protection: At temperatures above 650°C, the thin zinc coating evaporates
When manufacturing/use PLS steel elements pursuant to the quickly as zinc oxide (ZnO), causing fumes. When inhaled for a
generally recognized rules of engineering there are no prolonged period of time, ZnO fumes can cause metal fume
measures to be taken which are going beyond the public fever (diarrhoea, fever, dry throat), whereby these symptoms
occupational health and safety. normally disappear within 1 to 2 days after inhalation. The
The manufacturing/using of the PLS steel elements, pursuant critical temperature (failure temperature of the component)
to the generally recognized rules of engineering does not depends primarily on the component load, the static scheme
release substantial environmental pollutants. Particular ('rope effect') and the fire insulation of the component.
measures to protect the environment are not required. The
plasma cutting, welding, painting and hot dip galvanization
activities must respect the respective national regulations for Water
health and safety Galvanized steel is not soluble in water and does not release
any substances when exposed to water.
Residual material:
During processing residual pieces as well as turnings are to be Mechanical destruction
separately collected. This scrap steel is entirely recycled by Due to the ductility of steel, PLS steel elements react resiliently
melting and producing new steel products. in the event of unforeseeable mechanical destruction: In case
The recovered zinc can be used again for hot-dip galvanizing. of tensile load necking will occur before cracking. In case of a
lasting high compression load, components of steel may buckle
2.9 Packaging
or bulge. No splintering or breaking edges shall result.
Structural PLS elements are delivered in unpacked bindles. A
bundle of several PLS profiles is strapped with steel straps. To 2.14 Re-use phase
facilitate loading/unloading and protect during transportation, General:
the material is generally stacked with wooden battens in PLS steel elements are recyclable by 100 %. Due to the
between them. For sea transport, special packaging to protect magnetic properties of steel, >99 % of the used steel is
the goods while at sea might be used. regained after dismantling (European Commission Technical
Steel Research).
2.10 Condition of use
PLS elements are made from steel grades which are non- /low-
Re-use
alloyed steel products generated by alloying iron with other
PLS steel elements can be re-used. Currently, around 11 % of
metals and nonmetals (esp. carbon). Iron is the main
the products are re-used after dismantling.
component of steel sections and plates. The components are
listed under chapter 2.5 'Base materials'. During usage, no
Recycling:
changes in material composition shall occur.
PLS steel elements can be recycled without any problems after
dismantling. Currently, around 88 % of the products are used
PLS elements have a zinc layer, whose thickness is normalized
for closed-loop recycling (including 1 % loss). Data from
in EN ISO 1461.
industry estimates based on the following sources: European
Commission Technical Steel Research and Bundesministerium
2.11 Environment and health during use
für Umwelt, Naturschutz, Bau und Reaktorsicherheit.
The intended use of PLS elements does not hazard health or
the environment in any known way. If used properly, there are 2.15 Disposal
no known negative impacts of galvanized PLS sections on the
Due to its high value as a resource, steel scrap is not disposed,
environment or on the health of people.
but instead fed into a well-established cycle of reuse or
recycling. However, in case of dumping due to collection loss
2.12 Reference service life
no environmental impacts are expected.
In general, the reference service life is not relevant for
consideration of the LCA. As construction products with many
Waste code according to European Waste Catalogue: 17 04 05
different applications, a reference service life for structural PLS
- iron and steel
steel elements is not declared here. The purpose, possible
corrosion protection and adequate maintenance are decisive 2.16 Further information
for service life. Galvanizing allows for durable corrosion
Additional information on constructing with PRS and with steel
protection of PLS steel components under atmospheric
in general can be obtained from many public sources, for
corrosion conditions. The protection normally lasts for several
example:
decades without any need for maintenance or repair. For more
information regarding the reference service life of hot-dip • Astron.biz
galvanized structural steel, see ISO 14713-1. • bauforumstahl.de
• cticm.com
2.13 Extraordinary effects • bouwenmetstaal.nl
Fire • steel-sci.com
The material is class A1, i.e. not flammable per EN 13501.
3. LCA: Calculation rules
3.1 Declared Unit
3 Environmental Product Declaration - Astron Buildings S.A. - Astron PLS Product (cold-formed steel elements made of galvanized steel sheets)
The declared unit is 1 t of PLS cold-formed steel elements boundary related to the recycling of steel, which results from
made of galvanized steel sheets. the treatment of recycled materials from the point of end-of-
waste status to the point of substitution (as loads) and the
Declared unit and mass reference
substitution of primary resources (as benefits).
Name Value Unit
It also includes the benefits and loads related to the energy
Declared unit 1000 kg recovery from wooden wastes in a municipal waste incineration
Gross density 7850 kg/m3 plant as modelled in Module A5.
Only net flows leaving the product system are considered in
3.2 System boundary module D. The recycled content and the assumed processing
losses (e.g., during remelting) are taken from respective
Type of the EPD: cradle to gate with options, with modules C1–
ecoinvent 3 datasets; these parameters are used to estimate
C4, and module D.
the input of secondary material and compare it with the output
flows of the corresponding material.
The production of PRS structural steel (modules A1–A3)
includes raw material extraction, energy generation, waste
3.3 Estimates and assumptions
treatment and all transports up to the factory gate. In
No further assumptions and estimates relevant to the result had
accordance with COUNCIL REGULATION (EU) No 333/2011,
to be made beyond the points made in chapter 3 and in chapter
secondary steel is modelled as part of the product system from
4.
the moment they are available as unmixed scrap.
Waste or secondary fuels are not used for production. 3.4 Cut-off criteria
No data available from the company survey was neglected.
Module A4 is not declared due to large variances in transport
These include, among other things, material use, energy
distances between the production site and the construction site,
demand (heat, electricity), wooden battens for
where the product is installed.
storage/transport, consumables in production, waste treatment
and the transport of all inputs and outputs.
In module A5, the products are delivered to the construction
With this approach, mass and energy flows below 1 % were
site ready to be installed. Manual installation supported by a
also accounted for. No processes were neglected that would
diesel-powered mobile crane is assumed, electricity
have been known to the project managers and would have
consumption related to electric drilling machines, screwdrivers,
contributed significantly to the indicators of the impact
etc. is considered to be negligible.
assessment.
The wooden battens used for storage/transport are assumed to
be transported to an incineration plant; the recovered energy is 3.5 Background data
declared as exported energy. Ecoinvent v3.9.1, system model "cut-off by
classification" (2022) is used as the background database.
Modules B1 to B7 are not relevant for the declared products.
The indicator values of Modules B1 to B7 are thus 0 and not 3.6 Data quality
declared in the results table. The foreground data are based on extensive and detailed data
collection at the production site. The foreground data could be
In analogy to module A5, manual installation supported by a fully linked with corresponding data records from the
diesel-powered mobile crane is assumed (module C1). background database ecoinvent v3.9.1.
A share of 11 % of dismantled products is re-used in a different The background data was updated in 2022. Thus, the quality of
location and reaches the end-of-waste stage after dismantling the foreground and background data can be rated as very
(European Commission Technical Steel Research, 2001); the good.
corresponding amount leaves the product system as
'components for reuse'. 3.7 Period under review
The LCA data represents the production conditions for the Q4
In module C2, the remaining 89 % of the dismantled steel of year 2021 and Q1–Q3 of year 2022.
construction undergo a recycling (European Commission
3.8 Geographic Representativeness
Technical Steel Research, 2001) via a recycling platform, where
the steel is shredded and sorted. Land or region, in which the declared product system is
manufactured, used or handled at the end of the product´s
In module C3, shredding and sorting of the disassembled lifespan: Germany
product is assumed for the share to be recycled. The recovered
material leaves the product system as 'materials for recycling'.
3.9 Allocation
1 % of the shredded/sorted material is considered dust/loss,
No co-products are generated during the production of PLS
which is disposed of in a landfill for inert materials.
cold-formed steel elements made of galvanized steel sheets.
The net amounts of the metals leaving the product system are
Sorted production scrap is considered a secondary material
considered as 'use of secondary material' in Module D.
with no economic value (so no burdens allocated) and
considered closed-loop in modules A1–A3 (thus not taken into
As stated above, a reuse/recycling scenario in conformity with
account in module D.
the European Commission Technical Steel Research (2001) on
Economic allocation is applied to the blast furnace process
steel used in construction has been used. The landfilling of
related to pig iron and raw slag in accordance with the
shredding/sorting losses is declared in C3. Hence, no impacts
ecoinvent v3.9.1 dataset.
are declared in module C4.
No processes were modelled as part of the foreground model
Module D contains the benefits beyond the system boundary
that would have required an allocation of multi-input processes.
related to the reuse of the steel structure, leading to the
Background datasets on municipal waste incineration plants
substitution of the production of the corresponding steel
were taken from ecoinvent without any modification.
structure.
It also contains the benefits and loads beyond the system
Allocation of reuse, recycling and recovery was avoided by the
4 Environmental Product Declaration - Astron Buildings S.A. - Astron PLS Product (cold-formed steel elements made of galvanized steel sheets)
cut-off approach in the foreground model in line with EN 15804. the product-specific characteristics of performance, are taken
into account.
3.10 Comparability Ecoinvent v3.9.1, system model "cut-off by
Basically, a comparison or an evaluation of EPD data is only classification" (2022) is used as the background database.
possible if all the data sets to be compared were created
according to EN 15804 and the building context, respectively
4. LCA: Scenarios and additional technical information
Characteristic product properties of biogenic carbon Module C2
Note: 1 kg of biogenic carbon is equivalent to 44/12 kg of CO 2 In module C2, the remaining 89 % of the dismantled steel
construction undergo a recycling (European Commission
Information on describing the biogenic carbon content at
Technical Steel Research, 2001) via a recycling platform, where
factory gate
the steel is shredded and sorted.
Name ValueUnit
A default distance of 50 km to the shredding/sorting station is
kg assumed.
Biogenic carbon content in product -
C
Biogenic carbon content in accompanying kg Module C3
0.586
packaging C In module C3, a consumption of 0.015 kWh/kg of electricity for
shredding and sorting and 0.0437 MJ/kg of diesel fuel for
internal logistics are taken into for the shredding and sorting of
disassembled the product (values taken from published IBU
Module A5
EPD on identical product). The recovered material leaves the
In module A5, the products are delivered to the construction
product system as 'materials for recycling'.
site ready to be installed. Manual installation supported by a
1 % of the shredded/sorted material is considered dust/loss,
diesel-powered mobile crane is assumed, electricity
which is disposed of in a landfill for inert materials. A transport
consumption related to electric drilling machines, screwdrivers,
of 30 km.
etc. is considered to be negligible.
The net amounts of the metals leaving the product system are
The wooden battens used for storage/transport are assumed to
considered as 'use of secondary material' in Module D.
be transported 50 km with a lorry with a payload of 16-32 metric
ton, EURO6 to an incineration plant with an efficiency R1>0.6
Module D
(according to CEWEP Energy Report III); the recovered energy
Module D contains the benefits and loads beyond the system
is declared as exported energy; according to the same report,
boundary related to the recycling of metals, which result from
for its quantification, an efficiency of 28.3 % is assumed for the
the treatment of recycled materials from the point of end-of-
production of heat and 14.8 % for the production of electricity
waste status to the point of substitution (as loads) and the
(always referring to the lower heating value of the waste).
substitution of primary resources (as benefits).
It also includes the benefits and loads related to the energy
Module C1
recovery from wooden wastes in a municipal waste incineration
In analogy to module A5, manual installation supported by a
plant as modelled in Module A5.
diesel-powered mobile crane is assumed (module C1).
Only net flows leaving the product system are considered in
Electricity consumption related to electric drilling machines,
module D. The recycled content and the assumed processing
screw drivers, etc. is considered to be negligible.
losses (e.g., during remelting) are taken from respective
A share of 11 % of dismantled products is re-used in a different
ecoinvent 3 datasets; these parameters are used to estimate
location and reaches the end-of-waste stage after dismantling
the input of secondary material and compare it with the output
(European Commission Technical Steel Research, 2001); the
flows of the corresponding material.
corresponding amount leaves the product system as
"components for reuse".
5 Environmental Product Declaration - Astron Buildings S.A. - Astron PLS Product (cold-formed steel elements made of galvanized steel sheets)
5. LCA: Results
DESCRIPTION OF THE SYSTEM BOUNDARY (X = INCLUDED IN LCA; ND = MODULE OR INDICATOR NOT DECLARED; MNR =
MODULE NOT RELEVANT)
Benefits and
Construction loads beyond
Product stage Use stage End of life stage
process stage the system
boundaries
la ire ta m w a Ry lp p u s tro p s n a rT g n iru tc a fu n a M e h t m o rf tro p s n a rTe tis e h t o t e ta g y lb m e s s A e s U e c n a n e tn ia M ria p e R tn e m e c a lp e R tn e m h s ib ru fe R y g re n e la n o ita re p Oe s u re ta w la n o ita re p Oe s u n o itc u rts n o c -e Dn o itilo m e d tro p s n a rT g n is s e c o rp e ts a W la s o p s iD -e s u e R-y re v o c e R-g n ilc y c e Rla itn e to p
A1 A2 A3 A4 A5 B1 B2 B3 B4 B5 B6 B7 C1 C2 C3 C4 D
X X X MND X MND MND MNR MNR MNR MND MND X X X X X
RESULTS OF THE LCA - ENVIRONMENTAL IMPACT according to EN 15804+A2: 1 t of PLS cold-formed steel elements made
of galvanized steel sheets
Parameter Unit A1-A3 A5 C1 C2 C3 C4 D
GWP-total kg CO 2 eq 2.28E+03 7.39E+00 5.07E+00 8.23E+00 1.32E+01 0 -7.32E+02
GWP-fossil kg CO 2 eq 2.27E+03 5.23E+00 5.07E+00 8.22E+00 1.32E+01 0 -7.31E+02
GWP-biogenic kg CO 2 eq -2.15E+00 2.15E+00 0 0 0 0 0
GWP-luluc kg CO 2 eq 5.76E+00 6.46E-04 5.71E-04 4.06E-03 1.54E-03 0 -6.95E-01
ODP kg CFC11 eq 4.77E-05 8.42E-08 8.06E-08 1.79E-07 1.67E-07 0 -1.54E-05
AP mol H+ eq 1.57E+01 4.73E-02 4.7E-02 1.8E-02 5.81E-02 0 -3.77E+00
EP-freshwater kg P eq 1.4E-01 1.96E-05 1.83E-05 6.68E-05 4.63E-04 0 -3.77E-02
EP-marine kg N eq 2.39E+00 2.18E-02 2.18E-02 4.42E-03 2.14E-02 0 -6.82E-01
EP-terrestrial mol N eq 4.86E+01 2.38E-01 2.37E-01 4.61E-02 2.36E-01 0 -1.02E+01
kg NMVOC
POCP 1.06E+01 7.07E-02 7.01E-02 2.79E-02 7.06E-02 0 -3.76E+00
eq
ADPE kg Sb eq 3.05E-02 2.3E-06 1.77E-06 2.69E-05 9.57E-06 0 -8.22E-03
ADPF MJ 2.72E+04 6.87E+01 6.64E+01 1.17E+02 1.94E+02 0 -7.16E+03
m3 world eq
WDP 1.07E+03 1.52E-01 1.43E-01 4.81E-01 3.71E-01 0 -1.49E+02
deprived
GWP = Global warming potential; ODP = Depletion potential of the stratospheric ozone layer; AP = Acidification potential of land and water; EP =
Eutrophication potential; POCP = Formation potential of tropospheric ozone photochemical oxidants; ADPE = Abiotic depletion potential for non-fossil
resources; ADPF = Abiotic depletion potential for fossil resources; WDP = Water (user) deprivation potential)
RESULTS OF THE LCA - INDICATORS TO DESCRIBE RESOURCE USE according to EN 15804+A2: 1 t of PLS cold-formed
steel elements made of galvanized steel sheets
Parameter Unit A1-A3 A5 C1 C2 C3 C4 D
PERE MJ 2.61E+03 2.28E+01 3.73E-01 1.81E+00 1.22E+00 0 -6.42E+02
PERM MJ 2.24E+01 -2.24E+01 0 0 0 0 0
PERT MJ 2.64E+03 4.13E-01 3.73E-01 1.81E+00 1.22E+00 0 -6.42E+02
PENRE MJ 2.72E+04 6.87E+01 6.64E+01 1.17E+02 1.94E+02 0 -7.15E+03
PENRM MJ 0 0 0 0 0 0 0
PENRT MJ 2.72E+04 6.87E+01 6.64E+01 1.17E+02 1.94E+02 0 -7.15E+03
SM kg 5.01E+02 0 0 0 0 0 -5.51E+01
RSF MJ 0 0 0 0 0 0 0
NRSF MJ 0 0 0 0 0 0 0
FW m3 4.08E+01 1.11E-02 1.06E-02 3.05E-02 3.93E-02 0 -8.69E+00
PERE = Use of renewable primary energy excluding renewable primary energy resources used as raw materials; PERM = Use of renewable primary
energy resources used as raw materials; PERT = Total use of renewable primary energy resources; PENRE = Use of non-renewable primary energy
excluding non-renewable primary energy resources used as raw materials; PENRM = Use of non-renewable primary energy resources used as raw
materials; PENRT = Total use of non-renewable primary energy resources; SM = Use of secondary material; RSF = Use of renewable secondary fuels;
NRSF = Use of non-renewable secondary fuels; FW = Use of net fresh water
RESULTS OF THE LCA – WASTE CATEGORIES AND OUTPUT FLOWS according to EN 15804+A2:
1 t of PLS cold-formed steel elements made of galvanized steel sheets
Parameter Unit A1-A3 A5 C1 C2 C3 C4 D
HWD kg 2.56E-01 4.62E-04 4.47E-04 7.43E-04 5.26E-04 0 -8.1E-02
NHWD kg 1.29E+03 2.14E-01 1.18E-01 5.85E+00 9.33E+00 0 -3.13E+02
RWD kg 9.66E-02 1.38E-05 1.22E-05 6.7E-05 9.95E-04 0 9.22E-04
CRU kg 0 0 1.2E+02 0 0 0 0
MFR kg 0 0 0 0 8.81E+02 0 0
MER kg 0 0 0 0 0 0 0
EEE MJ 0 3.27E+00 0 0 0 0 0
EET MJ 0 6.26E+00 0 0 0 0 0
6 Environmental Product Declaration - Astron Buildings S.A. - Astron PLS Product (cold-formed steel elements made of galvanized steel sheets)
HWD = Hazardous waste disposed; NHWD = Non-hazardous waste disposed; RWD = Radioactive waste disposed; CRU = Components for re-use;
MFR = Materials for recycling; MER = Materials for energy recovery; EEE = Exported electrical energy; EET = Exported thermal energy
RESULTS OF THE LCA – additional impact categories according to EN 15804+A2-optional:
1 t of PLS cold-formed steel elements made of galvanized steel sheets
Parameter Unit A1-A3 A5 C1 C2 C3 C4 D
Disease
PM 2.12E-04 1.32E-06 1.31E-06 6.1E-07 1.08E-06 0 -5.45E-05
incidence
IR kBq U235 eq 7.42E+01 1.49E-02 1.36E-02 5.92E-02 4.17E-01 0 -1.22E+00
ETP-fw CTUe 0 0 0 0 0 0 0
HTP-c CTUh 2.18E-05 1.62E-09 1.55E-09 3.75E-09 2.85E-09 0 2.24E-06
HTP-nc CTUh 3.1E-05 1.23E-08 1.08E-08 8.29E-08 8.21E-08 0 -6.3E-06
SQP SQP 8.86E+03 5.66E+00 4.47E+00 7.06E+01 1.74E+01 0 -1.92E+03
PM = Potential incidence of disease due to PM emissions; IR = Potential Human exposure efficiency relative to U235; ETP-fw = Potential comparative
Toxic Unit for ecosystems; HTP-c = Potential comparative Toxic Unit for humans (cancerogenic); HTP-nc = Potential comparative Toxic Unit for humans
(not cancerogenic); SQP = Potential soil quality index
Disclaimer 1 – for the indicator “Potential Human exposure efficiency relative to U235”. This impact category deals mainly with the
eventual impact of low-dose ionizing radiation on human health of the nuclear fuel cycle. It does not consider effects due to possible
nuclear accidents, occupational exposure or radioactive waste disposal in underground facilities. Potential ionizing radiation from the
soil, radon and from some construction materials is also not measured by this indicator.
Disclaimer 2 – for the indicators “abiotic depletion potential for non-fossil resources”, “abiotic depletion potential for fossil resources”,
“water (user) deprivation potential, deprivation-weighted water consumption”, “potential comparative toxic unit for ecosystems”,
“potential comparative toxic unit for humans – cancerogenic”, “Potential comparative toxic unit for humans - not cancerogenic”,
“potential soil quality index”. The results of this environmental impact indicator shall be used with care as the uncertainties on these
results are high as there is limited experience with the indicator.
6. LCA: Interpretation
Figure 1 illustrates the relative contributions of the different
modules along the life cycle of the declared products The LCA is dominated by the manufacture of the product
(contribution of modules A1–C4 = 100 %). (modules A1–A3).
The benefits and burdens outside the product system vary in
significance depending on the indicator and fluctuate between -
10 % and -30 %.
The use of renewable primary energy is mainly caused by the
share of renewable energy in the electricity mix, thus the
production stage is the main driver of this impact category; the
same holds also for the use of non-renewable primary energy.
Material use of primary energy is comparably small and related
to the use of wooden battens used for transport and storage.
The material use of primary energy is transferred to its energy
use when the materials containing primary energy are
incinerated with energy recovery; the material use of primary
energy is subtracted from the material use indicator when the
materials containing primary energy are recycled. Non-
hazardous waste as the quantitatively most relevant waste
flows is mainly caused during mining and processing of metal
ores and related to the disposal of road infrastructure;
hazardous and radioactive waste are mainly caused by the
Figure 1: Relative contributions of the different life cycle
nuclear power in the electricity mix.
stages for cold-formed profiles (bended) (PLS) (modules
A1–C4 = 100 %)
7. Requisite evidence
7.1 Weathering For complete chemical weathering, recent publications (see
When exposed to the elements, the surfaces of hot-dip Hullmann 2003) quote corrosion rates for zinc of 3.0 g/m2*a
galvanized steel components become naturally covered in a (corresponding to approx. 0.5 µm/a).
protective layer known as patina. Patina is extremely durable Recent studies (BAST 2008 and Schröder 2013) examined hot-
and thus provides for exceptionally effective protection against dip galvanized steel crash barriers along the German Federal
corrosion, lasting several decades. Motorway BAB 4 and detected no measurable loss of thickness
At the same time, it protects the zinc coating, so that it remains of the zinc coating due to chemical weathering after 10 years of
intact for a long period of time. exposure to the elements.
The ever more stringent air quality improvement measures (in Chemical weathering can thus be assumed to be minimal and
particular the desulphurisation of power plant and engine fuels) therefore negligible, even over several years and under
have a major positive impact on the reduction of chemical increased corrosion stress such as along motorways (where
weathering of zinc coatings. Schröder 2013 reports of zinc deicing salt is used during the winter months).
coating depletion rates of up to 4.7 µm/a observed in the 1970s
in hot-dip galvanized steel crash barriers.
7 Environmental Product Declaration - Astron Buildings S.A. - Astron PLS Product (cold-formed steel elements made of galvanized steel sheets)
8. References
Product category rules of IBU
ISO 14025
IBU (2021) ISO 14025:2006-07, Environmental labels and declarations -
IBU (2021): PCR Part A: Calculation rules for the life cycle Type III Environmental declarations - Principles and
assessment and requirements on the project report according procedures.
to EN 15804+A2. Version 1.3, Institut Bauen und Umwelt e.V.,
Berlin. ISO 14044
EN ISO 14044:2006-07, Environmental management - Life
IBU (2021) cycle assessment - Requirements and guidance (ISO
IBU (2021): General Instructions for the EPD Programme of the 14044:2006); German and English versions EN ISO
Institut Bauen und Umwelt e.V. (General Instructions for the 14044:2006.
IBU EPD Programme). Version 2.0, Institut Bauen unf Umwelt,
Berlin. ISO 14713-1
DIN EN ISO 14713-1:2017-08, Zinc coatings - Guidelines and
IBU (2023) recommendations for the protection against corrosion of iron
IBU (2023): PCR Part B: Requirements on the EPD for and steel in structures - Part 1: General principles of design and
structural steel. Version 2023/04, Institut Bauen und Umwelt corrosion resistance (ISO 14713-1:2017); German version EN
e.V., Berlin. ISO 14713-1:2017.
Standards and legal documents EN 15804
DIN EN 15804+A2:2022-03, Sustainability of construction
EN 1090-1 works - Environmental product declarations - Core rules for the
DIN EN 1090-1:2012-02, Execution of steel structures and product category construction products; German version EN
aluminium structures - Part 1: Requirements for conformity 15804:2012+A2:2019 + AC:2021.
assessment of structural components; German version EN
1090-1:2009+A1:2011. EN 16485
DIN EN 16485:2014-07, Round and sawn timber -
EN 1090-2 Environmental Product Declarations - Product category rules
DIN EN 1090-2:2012-02, Execution of steel structures and for wood and wood-based products for use in construction;
aluminium structures - Part 2: Technical requirements for steel German version EN 16485:2014.
structures; German version EN 1090-2:2018.
ECHA candidate list
EN 1090-4 The Candidate List of substances of very high concern,
EN 1090-4 Execution of steel structures and aluminium available via https://echa.europa.eu/nl/-/four-newsubstances-
structures – Part 4: Technical requirements for cold-formed added-to-the-candidate-list.
structural steel elements and cold-formed structures for roof,
ceiling, floor and wall applications. ETA-18/1027
ETA-18/1027 of 19 November 2018 for Metal Frame Building
EN ISO 1461 Kits by Astron Buildings S.A.
DIN EN ISO 1461:2009-10, Hot dip galvanized coatings on
fabricated iron and steel articles - Specifications and test Regulation on biocidal products
methods (ISO 1461:2009); German version EN ISO 1461:2009. REGULATION (EU) No 528/2012 OF THE EUROPEAN
PARLIAMENT AND OF THE COUNCIL of 22 May 2012
EN 1993 concerning the making available on the market and use of
DIN EN 1993-1-1:2010-12, Eurocode 3: Design of steel biocidal products.
structures - Part 1-1: General rules and rules for buildings;
German version EN 1993-1-1:2005 + AC:2009. Regulation (EU) Nr. 305/2011(CPR)
REGULATION (EU) No 305/2011 OF THE EUROPEAN
EN 1994 PARLIAMENT AND OF THE COUNCIL of 9 March 2011 laying
DIN EN 1994-1-1:2010-12, Eurocode 4: Design of composite down harmonised conditions for the marketing of construction
steel and concrete structures - Part 1-1: General rules and rules products and repealing Council Directive 89/106/EEC.
for buildings; German version EN 1994-1-1:2004 + AC:2009.
Regulation on the European Waste List
ISO 9001 http://www.gesetze-im-internet.de/avv/anlage.html.
DIN EN ISO 9001:2015, Quality management systems -
Requirements. Additional references
EN 10025 BAST (2008)
DIN EN 10025-1:2005-02, Hot rolled products of structural BAST (2008): Coil-coated safety rails; German Federal
steels - Part 1: General technical delivery conditions; German Highway Research Institute (BASt) Bergisch-Gladbach 2008.
version EN 10025-1:2004.
Bundesministerium für Umwelt, Naturschutz, Bau und
ISO 12944-2 Reaktorsicherheit
DIN EN ISO 12944-2:2018-04, Paints and varnishes - Instrumente zur Wiederverwendung von Bauteilen und
Corrosion protection of steel structures by protective paint hochwertigen Verwertung von Baustoffen',
systems - Part 2: Classification of environments (ISO 12944- (Umweltforschungsplan des Bundesministeriums für Umwelt,
2:2017); German version EN ISO 12944-2:2017. Naturschutz, Bau und Reaktorsicherheit ; Forschungskennzahl
8 Environmental Product Declaration - Astron Buildings S.A. - Astron PLS Product (cold-formed steel elements made of galvanized steel sheets)
3712 32 319; UBA-FB 002208). European Commission Technical Steel Research (2001)
Sansom M., Meijer J. (2001): Life-cycle assessment; (LCA) for
CEWEP Energy Report III (2013) steel construction, European Commission technical steel
Reimann D.O. (2013): CEWEP Energy Report III (Status 2007 research.
– 2010); Results of Specific Data for Energy, R1 Plant
Efficiency Factor and NCV of 314 European Waste-to-Energy Hullmann 2003
(WtE) Plants. CEWEP, Würzburg/Brussels, 2013. Hullmann H. (2003): Natürlich oxidierende Metalloberflächen;
Umweltauswirkungen beim Einsatz von Kupfer und Zink in
DASt-Guideline 022 Gebäudehüllen; 2003, Stuttgart, Fraunhofer ISB-Verlag, ISBN:
Institut Feuerverzinken (2016): Feuerverzinken von tragenden 3-8167-6218-2.
Stahlbauteilen. DASt-Richtlinie 022 und Erläuterung zur DASt-
Richtlinie 022. Institut Feuerverzinken, Ausgabe Juni 2016. Schröder 2013
Schröder M. (2012): Korrosionsbeständigkeit von
ecoinvent v3.9.1 diskontinuierlich und kontinuierlich verzinkten Schutzplanken,
ecoinvent v3.9.1, LCA database, 12/2022. Ecoinvent centre, Vortrag anlässlich EGGA-Assembly, 10.-13. Juni 2013,
Zürich. Dresden.
9 Environmental Product Declaration - Astron Buildings S.A. - Astron PLS Product (cold-formed steel elements made of galvanized steel sheets)
Publisher
Institut Bauen und Umwelt e.V. +49 (0)30 3087748- 0
Hegelplatz 1 info@ibu-epd.com
10117 Berlin www.ibu-epd.com
Germany
Programme holder
Institut Bauen und Umwelt e.V. +49 (0)30 3087748- 0
Hegelplatz 1 info@ibu-epd.com
10117 Berlin www.ibu-epd.com
Germany
Author of the Life Cycle Assessment
Dr. Frank Werner - Umwelt & Entwicklung + 41 (0)44 241 39 06
Kammelenbergstrasse 30 frank@frankwerner.ch
9011 St. Gallen http://www.frankwerner.ch/
Switzerland
Owner of the Declaration
Astron Buildings S.A +352 802 91-1
Route d’Ettelbruck 34 info@astron.biz
9230 Diekirch www.astron.biz
Luxembourg
10 Environmental Product Declaration - Astron Buildings S.A. - Astron PLS Product (cold-formed steel elements made of galvanized steel sheets)
