ENVIRONMENTAL PRODUCT DECLARATION
as per ISO 14025 and EN 15804+A2
Owner of the Declaration dormakaba International Holding GmbH
Publisher Institut Bauen und Umwelt e.V. (IBU)
Programme holder Institut Bauen und Umwelt e.V. (IBU)
Declaration number EPD-DOR-20220359-CBA4-EN
Issue date 15.03.2023
Valid to 14.03.2028
Automatic Sliding Door ST FLEX Green
dormakaba
www.ibu-epd.com | https://epd-online.com
General Information
dormakaba Automatic Sliding Door ST FLEX Green
Programme holder Owner of the declaration
IBU – Institut Bauen und Umwelt e.V. dormakaba International Holding GmbH
Hegelplatz 1 DORMA Platz 1
10117 Berlin 58256 Ennepetal
Germany Germany
Declaration number Declared product / declared unit
EPD-DOR-20220359-CBA4-EN The declared unit is one piece (1 pc.) of the ST FLEX Green automatic
sliding door system without drive comprising:
• ST FLEX Green sliding panels,
• ST FLEX Green side screens and
• product packaging
This declaration is based on the product category rules: Scope:
Automatic doors, automatic gates, and revolving door systems, This EPD refers to the entire life cycle of a specific ST FLEX Green
01.08.2021 automatic sliding door system.
(PCR checked and approved by the SVR) The production location is dormakaba Zusmarshausen, Germany. Green
electricity is used a the production facility. The material and energy flows
were taken into consideration accordingly.
Issue date
The year of data collection is 2022.
15.03.2023
The owner of the declaration shall be liable for the underlying information
and evidence; the IBU shall not be liable with respect to manufacturer
information, life cycle assessment data and evidences.
Valid to
14.03.2028 The EPD was created according to the specifications of EN 15804+A2. In
the following, the standard will be simplified as EN 15804.
Verification
The standard EN 15804 serves as the core PCR
Independent verification of the declaration and data according to ISO
14025:2011
internally X externally
Dipl.-Ing. Hans Peters
(Chairman of Institut Bauen und Umwelt e.V.)
Florian Pronold Dr.-Ing. Wolfram Trinius,
(Managing Director Institut Bauen und Umwelt e.V.) (Independent verifier)
1 Environmental Product Declaration - dormakaba - Automatic Sliding Door ST FLEX Green
Product
Product description/Product definition Base materials/Ancillary materials
The ST FLEX Green stands for an automatic sliding door Performance data of the product with respect to its
system manufactured by dormakaba. dormakaba underlines its characteristics in accordance with the relevant technical
contribution to more energy efficiency and more sustainability provision which can be applied are mentioned above.
with the sliding door ST FLEX Green. The automatic sliding The ST FLEX Green Automatic Sliding Door comprises the
door has a slim, thermal divided profile system on basis of the following components including packaging:
ST FLEX profile.
Therefore, heat insulation is achieved without compromising in
the slim profile. ST FLEX Green makes considerable savings of
the running energy and heating costs possible, as well as a
reduction in CO2- emissions for the entire use phase.
To meet all requirements, the ST FLEX Green system can be
combined with different ES operator versions, among others ES
PROLINE and ES 200. For the Sliding Door ST Flex Green the
standards which can be applied are the following:
• EN 16005
• DIN 18650-1/ -2
• ISO 13849-1
• EN 60335-1
• EN 60335-2-103
• IEC 60335-2-103
• 2011/65/EU (RoHS)
The product contains partial articles which contain substances
Application listed in the Candidate List of REACH Regulation
The ST FLEX Green automatic sliding door system is used in 1907/2006/EC (date: 17.01.2023) exceeding 0.1 percentage by
particular where energy saving enjoys key significance during mass: no
the reference service life. Each system is manufactured to the
individual dimensions of the respective building project. The Candidate List can be found on the ECHA website
address: https://echa.europa.eu/de/home.
Technical Data
Following data are applicable for the sliding panels and side Reference service life
screens: The reference service life amounts to 10 years, depending on
the application and frequency of use. Regular maintenance is
• Heat transition coeffizient (U-value) for the sliding door
advised to ensure the life expactancy of 10 years. For repairs
system measuring 6250 x 3305: 1,4 [W/m²K]
and renewals, suitable spare parts are available. The ST FLEX
• Heat transition coeffizient (U-value) for the sliding door
Green is tested and certified, meaning they are desingned to
system measuring 2100 x 2205: 1,6 [W/m²K]
withstand a minimum of 1.000.000 cycles.
• Insulation glass units: 1,0 [W/m²K]
LCA: Calculation rules
Declared Unit Construction stage - Modules A4-A5
The declared unit is 1 piece of the product: Automatic Sliding The construction process stage includes:
Door ST FLEX Green — A4, transport to the building site;
Declared unit and mass reference — A5, installation into the building; including provision of all
materials, products and energy, as well as waste processing up
Name Value Unit
to the end-of waste state or disposal of final residues during the
Declared unit 1 pce.
construction process stage.
Mass (total system) 287.43 kg
Use stage - Module B6
System boundary The use stage related to the operation of the building includes:
The type of EPD is: cradle-to-gate with options, modules C1– — B6, operational energy use
C4, and module D (A1–A3 + C + D and additional modules: A4
+ A5 + B6) End-of-life stage– Modules C1-C4 and D
The end-of-life stage includes:
Production - Module A1-A3 — C1, de-construction, demolition:
The product stage includes: — C2, transport to waste processing;
— A1, raw material extraction, processing and mechanical — C3, waste processing for reuse, recovery and/or recycling;
treatments, processing of secondary material input (e.g. — C4, disposal; including provision and all transport, provision
recycling processes), of all materials, products and related energy and water use.
— A2, transport to the manufacturer, Module D (Benefits and loads beyond the system boundary)
— A3, manufacturing and assembly including provision of all includes:
materials, products and energy, as well as waste processing up — D, recycling potentials, expressed as net impacts and
to the end-of waste state. benefits.
2 Environmental Product Declaration - dormakaba - Automatic Sliding Door ST FLEX Green
Geographic Representativeness Comparability
Land or region, in which the declared product system is Basically, a comparison or an evaluation of EPD data is only
manufactured, used or handled at the end of the product´s possible if all the data sets to be compared were created
lifespan: Global according to EN 15804 and the building context, respectively
the product-specific characteristics of performance, are taken
into account. Background database: GaBi, SP40.
LCA: Scenarios and additional technical information
End of life (C1-C4)
Characteristic product properties of biogenic carbon
C1: The product expansion depends on the building. The
Information on describing the biogenic Carbon Content at product share is so low that no environmental burden is
factury gate assumed.
Name ValueUnit C2: Transport to waste treatment at end of life is 50km.
Biogenic carbon content in accompanying kg Name Value Unit
0.003
packaging C Collected separately waste type waste type 278 kg
Reuse - kg
The following technical scenario information is required for the Recycling 36.4 kg
declared modules.
Energy recovery 7.59 kg
Transport to the building site (A4) Landfilling 234 kg
Name Value Unit Transport to waste management 50 km
Litres of fuel (per 1 kg) 0.00276 l/100km
The product is disassembled in a recycling process. Material
Transport distance via medium truck 100 km recycling is then assumed for the metals, electronics and
Capacity utilisation (including empty runs) 55 % electromechanics. The plastic components are assumed to be
incinerated with energy recovery. Glass and minor proportions
Transport distance is declared for a distance of 100km by truck
of residues arising from the recycling process are landfilled.
in order to allow scaling to a specific point of installation.
Region for the End of Life is: Global.
Installation into the building (A5)
Reuse, recovery and/or recycling potentials (D), relevant
Name Value Unit
scenario information
Waste packaging (paper and plastic) 9 kg The collection rate is 100%.
Reference service life Name Value Unit
Recycling 100 %
Name Value Unit
Life Span according to the manufacturer 10 a
Operational energy use (B6)
The drive unit is not included in this EPD, which is why B6 is
not declared. The results for the drive unit are shown in a
separate EPD.
3 Environmental Product Declaration - dormakaba - Automatic Sliding Door ST FLEX Green
LCA: Results
DESCRIPTION OF THE SYSTEM BOUNDARY (X = INCLUDED IN LCA; MND = MODULE OR INDICATOR NOT DECLARED; MNR
= MODULE NOT RELEVANT)
Benefits and
Construction loads beyond
Product stage Use stage End of life stage
process stage the system
boundaries
la ire ta m w a Ry lp p u s tro p s n a rT g n iru tc a fu n a M e h t m o rf tro p s n a rTe tis e h t o t e ta g y lb m e s s A e s U e c n a n e tn ia M ria p e R tn e m e c a lp e R tn e m h s ib ru fe R y g re n e la n o ita re p Oe s u re ta w la n o ita re p Oe s u n o itc u rts n o c -e Dn o itilo m e d tro p s n a rT g n is s e c o rp e ts a W la s o p s iD -e s u e R-y re v o c e R-g n ilc y c e Rla itn e to p
A1 A2 A3 A4 A5 B1 B2 B3 B4 B5 B6 B7 C1 C2 C3 C4 D
X X X X X MND MND MNR MNR MNR MND MND X X X X X
RESULTS OF THE LCA - ENVIRONMENTAL IMPACT according to EN 15804+A2: 1 piece Automatic Sliding Door ST FLEX
Green
Parameter Unit A1-A3 A4 A5 C1 C2 C3 C4 D
GWP-total kg CO 2 eq 5.1E+02 2.51E+00 2.29E+01 0 1.22E+00 1.93E+01 3.58E+00 -6.37E+01
GWP-fossil kg CO 2 eq 5.07E+02 2.4E+00 2.29E+01 0 1.16E+00 1.93E+01 3.56E+00 -6.35E+01
GWP-biogenic kg CO 2 eq 2.25E+00 1.11E-01 5.33E-04 0 5.4E-02 4.5E-04 1.2E-02 -1.79E-01
GWP-luluc kg CO 2 eq 1.97E-01 5.72E-05 1E-03 0 2.77E-05 1E-03 1E-02 -2E-02
ODP kg CFC11 eq 3.11E-09 2.54E-16 1.15E-14 0 1.23E-16 9.73E-15 1.32E-14 -3.36E-10
AP mol H+ eq 3.35E+00 2E-03 4E-03 0 1E-03 3E-03 2.6E-02 -1.89E-01
EP-freshwater kg P eq 4.72E-04 5.14E-07 1.84E-06 0 2.49E-07 1.55E-06 6.11E-06 -4.49E-05
EP-marine kg N eq 7.46E-01 7.65E-04 9.18E-04 0 3.71E-04 7.75E-04 7E-03 -2.8E-02
EP-terrestrial mol N eq 8.5E+00 9E-03 1.9E-02 0 4E-03 1.6E-02 7.2E-02 -3.08E-01
kg NMVOC
POCP 1.62E+00 2E-03 3E-03 0 1E-03 2E-03 2E-02 -8.8E-02
eq
ADPE kg Sb eq 2.46E-04 7.21E-08 1.58E-07 0 3.49E-08 1.34E-07 3.19E-07 -6.18E-05
ADPF MJ 7.32E+03 3.41E+01 1.06E+01 0 1.65E+01 8.95E+00 4.67E+01 -9.55E+02
m3 world eq
WDP 3.07E+01 5E-03 2.34E+00 0 2E-03 1.97E+00 3.73E-01 -3.98E+00
deprived
GWP = Global warming potential; ODP = Depletion potential of the stratospheric ozone layer; AP = Acidification potential of land and water; EP =
Eutrophication potential; POCP = Formation potential of tropospheric ozone photochemical oxidants; ADPE = Abiotic depletion potential for non-fossil
resources; ADPF = Abiotic depletion potential for fossil resources; WDP = Water (user) deprivation potential)
RESULTS OF THE LCA - INDICATORS TO DESCRIBE RESOURCE USE according to EN 15804+A2: 1 piece Automatic Sliding
Door ST FLEX Green
Parameter Unit A1-A3 A4 A5 C1 C2 C3 C4 D
PERE MJ 7.88E+02 1.07E-01 2.76E+00 0 5.2E-02 2.33E+00 6.11E+00 -3.52E+02
PERM MJ 0 0 0 0 0 0 0 0
PERT MJ 7.88E+02 1.07E-01 2.76E+00 0 5.2E-02 2.33E+00 6.11E+00 -3.52E+02
PENRE MJ 6.77E+03 3.41E+01 3.98E+02 0 1.65E+01 1.73E+02 4.67E+01 -9.56E+02
PENRM MJ 5.51E+02 0 -3.87E+02 0 0 -1.64E+02 0 0
PENRT MJ 7.32E+03 3.41E+01 1.06E+01 0 1.65E+01 8.95E+00 4.67E+01 -9.56E+02
SM kg 2.86E+01 0 0 0 0 0 0 0
RSF MJ 0 0 0 0 0 0 0 0
NRSF MJ 0 0 0 0 0 0 0 0
FW m3 1.75E+00 1.93E-04 5.6E-02 0 9.34E-05 4.7E-02 1.2E-02 -5.83E-01
PERE = Use of renewable primary energy excluding renewable primary energy resources used as raw materials; PERM = Use of renewable primary
energy resources used as raw materials; PERT = Total use of renewable primary energy resources; PENRE = Use of non-renewable primary energy
excluding non-renewable primary energy resources used as raw materials; PENRM = Use of non-renewable primary energy resources used as raw
materials; PENRT = Total use of non-renewable primary energy resources; SM = Use of secondary material; RSF = Use of renewable secondary fuels;
NRSF = Use of non-renewable secondary fuels; FW = Use of net fresh water
RESULTS OF THE LCA – WASTE CATEGORIES AND OUTPUT FLOWS according to EN 15804+A2:
1 piece Automatic Sliding Door ST FLEX Green
Parameter Unit A1-A3 A4 A5 C1 C2 C3 C4 D
HWD kg 1.26E-05 3.31E-09 4.04E-08 0 1.6E-09 3.41E-08 7.11E-07 -2.51E-06
NHWD kg 6.46E+01 3E-03 2.38E+00 0 2E-03 2E+00 2.35E+02 -1.12E+01
RWD kg 1.6E-01 3.66E-05 3.94E-04 0 1.77E-05 3.32E-04 5.31E-04 -9E-02
CRU kg 0 0 0 0 0 0 0 0
MFR kg 0 0 0 0 0 9.16E+00 0 0
MER kg 0 0 0 0 0 0 0 0
EEE MJ 0 0 4.24E+01 0 0 0 0 0
4 Environmental Product Declaration - dormakaba - Automatic Sliding Door ST FLEX Green
EET MJ 0 0 9.73E+01 0 0 0 0 0
HWD = Hazardous waste disposed; NHWD = Non-hazardous waste disposed; RWD = Radioactive waste disposed; CRU = Components for re-use;
MFR = Materials for recycling; MER = Materials for energy recovery; EEE = Exported electrical energy; EET = Exported thermal energy
RESULTS OF THE LCA – additional impact categories according to EN 15804+A2-optional:
1 piece Automatic Sliding Door ST FLEX Green
Parameter Unit A1-A3 A4 A5 C1 C2 C3 C4 D
Disease
PM 2.1E-05 1.26E-08 5.2E-08 0 6.12E-09 4.38E-08 3.16E-07 -2.86E-06
incidence
IR kBq U235 eq 2.63E+01 5E-03 3.5E-02 0 3E-03 3E-02 5.5E-02 -1.74E+01
ETP-fw CTUe 8.57E+03 2.42E+01 3.98E+00 0 1.17E+01 3.36E+00 2.67E+01 -2.93E+02
HTP-c CTUh 2.66E-07 4.54E-10 3.45E-10 0 2.2E-10 2.91E-10 3.95E-09 -1.46E-08
HTP-nc CTUh 4.89E-06 1.94E-08 3.49E-08 0 9.41E-09 2.94E-08 4.35E-07 -4.32E-07
SQP SQP 4.19E+02 8.8E-02 3.18E+00 0 4.2E-02 2.68E+00 9.73E+00 -6.51E+01
PM = Potential incidence of disease due to PM emissions; IR = Potential Human exposure efficiency relative to U235; ETP-fw = Potential comparative
Toxic Unit for ecosystems; HTP-c = Potential comparative Toxic Unit for humans (cancerogenic); HTP-nc = Potential comparative Toxic Unit for humans
(not cancerogenic); SQP = Potential soil quality index
Disclaimer 1 – for the indicator “Potential Human exposure efficiency relative to U235”. This impact category deals mainly with the
eventual impact of low-dose ionizing radiation on human health of the nuclear fuel cycle. It does not consider effects due to possible
nuclear accidents, occupational exposure or radioactive waste disposal in underground facilities. Potential ionizing radiation from the
soil, radon and from some construction materials is also not measured by this indicator.
Disclaimer 2 – for the indicators “abiotic depletion potential for non-fossil resources”, “abiotic depletion potential for fossil resources”,
“water (user) deprivation potential, deprivation-weighted water consumption”, “potential comparative toxic unit for ecosystems”,
“potential comparative toxic unit for humans – cancerogenic”, “Potential comparative toxic unit for humans - not cancerogenic”,
“potential soil quality index”. The results of this environmental impact indicator shall be used with care as the uncertainties on these
results are high as there is limited experience with the indicator.
References
Standards declarations — Type III environmental declarations —
Principles and procedures
DIN 18650-1
DIN 18650-1: 2010-06,Powered pedestrian doors –Part 1: Further References
Product requirements and test methods.
European Chemicals Agency (ECHA)
DIN 18650-2 https:echa.europa.eu/de/home
DIN 18650-2:2010-06, Powered pedestrian doors –Part 2:
Safety at powered pedestrian doors. GaBi ts software
Sphera Solutions GmbH Gabi Software System and Database
EN 15804 for Life CyclenEngineering 1992-2020 Version 10.0.0.71
EN 15804:2012-04, Sustainability of construction works – University of Stuttgart Leinfelden-Echterdingen
Environmental product declarations – Core rules for the product
category of construction products; German version EN GaBi ts documentation
15804:2012. GaBi life cycle inventory data documentation
(https://www.gabisoftware.com/support/gabi/gabidatabase-
EN 16005 2020-lci-documentation/).
EN 16005:2013-01, Power operated pedestrian doorsets -
Safety in use - Requirements and test methods; German IBU 2021
version EN 16005:2012 General Instructions for the EPD programme of Institut Bauen
und Umwelt e.V. Version 2.0, Berlin: Institut Bauen und Umwelt
EN 60335-1 e.V., 2021.
EN 60335-1; VDE 0700-1:2012-10:2012-10, Household and www.ibu-epd.com
similar electrical appliances – Safety - Part 1: General
requirements (IEC 60335-1:2010, modified); German version LCA-tool dormakaba
EN 60335-1:2012. LCA tool, ENS doors LCA tool no.: BU-DOR-202107-LT1-EN
Developed by Sphera Solutions GmbH.
EN 60335
EN 60335-2-103/A1; Household and similar electrical PCR Part A
appliances - Safety - Part 2-103: Particularrequirements for PCR – Part A: Calculation Rules for the Life Cycle Assessment
drives for gates, doors and windows (IEC 61/2863/CDV:2005); and Requirements on the Project Re-port according to EN
German version EN 60335-2-103:2003/prA1:2005.2011/65/EU 15804+A2:2019, Version 1.0, Institut Bauen und Umwelt e.V.,
www.ibu-epd.com.
ISO 13849-1
ISO 13849-1:2008-12, Safety of machinery – Safetyrelated PCR Part B
parts of control systems – Part 1: General principles for design PCR – Part B: Requirements on the EPD for Automatic doors,
(ISO 13849-1:2006. automatic gates, and revolving door systems, 08/2021, Institut
Bauen und Umwelt e.V., www.ibu-epd.com
ISO 14025
DIN EN ISO 14025:201110, Environmental labels and
5 Environmental Product Declaration - dormakaba - Automatic Sliding Door ST FLEX Green
ROHS3 Directive
REACH Regulation Directive 2011/65/EU of the European Parliament and of the
REACH Regulation (EC) No 1907/2006 of the European Council of 8 June 2011 on the restriction of the use of certain
Parliament and of the Council on the Registration, Evaluation, hazardous substances in electrical and electronic equipment
Authorisation and Restriction of Chemicals.
6 Environmental Product Declaration - dormakaba - Automatic Sliding Door ST FLEX Green
Publisher
Institut Bauen und Umwelt e.V. +49 (0)30 3087748- 0
Hegelplatz 1 info@ibu-epd.com
10117 Berlin www.ibu-epd.com
Germany
Programme holder
Institut Bauen und Umwelt e.V. +49 (0)30 3087748- 0
Hegelplatz 1 info@ibu-epd.com
10117 Berlin www.ibu-epd.com
Germany
Author of the Life Cycle Assessment
dormakaba International Holding GmbH +49 2333 793-0
DORMA Platz 1 info.de@dormakaba.com
58256 Ennepetal www.dormakaba.com
Germany
Owner of the Declaration
dormakaba International Holding GmbH +49 2333 793-0
DORMA Platz 1 info.de@dormakaba.com
58256 Ennepetal www.dormakaba.com
Germany
7 Environmental Product Declaration - dormakaba - Automatic Sliding Door ST FLEX Green
