ENVIRONMENTAL PRODUCT DECLARATION
as per ISO 14025 and EN 15804+A2
Owner of the Declaration dormakaba International Holding GmbH
Publisher Institut Bauen und Umwelt e.V. (IBU)
Programme holder Institut Bauen und Umwelt e.V. (IBU)
Declaration number EPD-DOR-20240077-CBA1-EN
Issue date 04.03.2024
Valid to 03.03.2029
Automatic Swing Door Operator ED 900
dormakaba
www.ibu-epd.com | https://epd-online.com
General Information
dormakaba Automatic Swing Door Operator ED 900
Programme holder Owner of the declaration
IBU – Institut Bauen und Umwelt e.V. dormakaba International Holding GmbH
Hegelplatz 1 DORMA Platz 1
10117 Berlin 58256 Ennepetal
Germany Germany
Declaration number Declared product / declared unit
EPD-DOR-20240077-CBA1-EN 1 piece of the product: Automatic Swing Door Operator ED 900, consisting
of the following items:
- ED 900 swing door operator
- ED slide channel set
- ED basic cover
- Product packaging
This declaration is based on the product category rules: Scope:
Drive systems for automatic doors and gates, 01.08.2021 This Environmental Product Declaration refers to a specific automatic
(PCR checked and approved by the SVR) swing door operator manufacutred by dormakaba. The production site is
located in Ennepetal (Germany). Green electricity is being used at the
production site.
Issue date
Data represents the year 2022.
04.03.2024
The owner of the declaration shall be liable for the underlying information
and evidence; the IBU shall not be liable with respect to manufacturer
information, life cycle assessment data and evidences.
Valid to
03.03.2029 The EPD was created according to the specifications of EN 15804+A2. In
the following, the standard will be simplified as EN 15804.
Verification
The standard EN 15804 serves as the core PCR
Independent verification of the declaration and data according to ISO
14025:2011
internally X externally
Dipl.-Ing. Hans Peters
(Chairman of Institut Bauen und Umwelt e.V.)
Florian Pronold Dr.-Ing. Wolfram Trinius,
(Managing Director Institut Bauen und Umwelt e.V.) (Independent verifier)
1 Environmental Product Declaration - dormakaba - Automatic Swing Door Operator ED 900
Product
Name Value Unit
Product description/Product definition
Height 240 mm
The automatic swing door operator is designed for single- or
Installation depth 152 mm
double leaf doors. The operator can be mounted with standard
arm as push-version and with slide channel as pull-version. Maximum door weight ED 100 272 kg
Apart from the extended cover, an integrated door coordinator Opening speed maximum 50 cm/s
is also available for double-leaf operators. By using the Closing speed maximum 40 cm/s
dormakaba upgrade card, the functional scope can be adapted
Hold open time maximum 60 s
to a variety of door situations.
Supply voltage, frequency maximum 60 Hz
Features Power consumption 175 W
Class of protection 20 IP
• Flexible configuration of the functions actually required
• Inexpensive transport and easy assembly thanks to Performance data of the product with respect to its
lower weights characteristics in accordance with the relevant technical
• Low-noise application thanks to multi-stage gear provision which can be applied are mentioned above.
• Elegant design: dormakaba Contur Design with an
operator height of only 70 mm Base materials/Ancillary materials
The major material composition including the packaging of the
For the use and application of the product the respective product is listed below.
national provisions at the place of use apply: Name Value Unit
• ISO 13849-1 Steel 33 %
• DIN 18650-1 Aluminium 19 %
• DIN 18650-2
Paper 14 %
• EN 16005
Zinc 14 %
• EN 60335-1
• 2011/65/EU ROHS3 Directive Plastic 10 %
• Machinery Directive 2006/42/EC Electronics 9 %
Brass 1 %
The CE-marking takes into account the proof of conformity with
The ED 900 includes partial articles which contain substances
the respective harmonized standards based on the legal
listed in the Candidate List of REACH Regulation
provisions above.
1907/2006/EC (date: 23.01.2024) exceeding 0.1 percentage by
Application mass: yes
dormakaba swing door operators are suitable for various • Lead (Pb): 7439-92-1 (CAS-No) is used in the steel
applications: alloy. The concentration of lead in the alloy does not
• For single- or double- leaf swing doors exceed 0,35% (by mass).
• Assembly on smoke or fire doors: as pull- version with The Candidate List can be found on the ECHA website
slide channels and as push- version with standard arm address: https:echa.europa.eu/de/home.
• Automation of doors with low traffic capacity (Low-
Reference service life
Energy Mode) and heavily frequented doors (Full-
The reference service life of the ED 900 amounts to 10 years
Energy Mode)
and depends on the application and frequency of use. Regular
• High torque for full-automatic swing doors with radar
maintenance is advised to ensure the life expectancy of 10
detector control
years. For repairs or renewals, suitable spare parts are
• Suitable for internal and external door
available. The swing door operators are tested and certified to
Technical Data EN 16005, meaning they are designed to withstand a minium of
The ED 900 has the following technical properties: 1.000.000 cycles.
LCA: Calculation rules
— A1, raw material extraction, processing and mechanical
Declared Unit treatments, processing of secondary material input (e.g.
recycling processes),
The declared unit is 1 piece of the product: ED 900 — A2, transport to the manufacturer,
Name Value Unit — A3, manufacturing and assembly including provision of all
materials, products and energy, as well as waste processing up
Declared unit 1 pce.
to the end-of waste state.
Mass reference 13.54 kg/pce
Construction stage - Modules A4-A5
System boundary
The construction process stage includes:
The type of EPD is: cradle to gate with options, modules C1– — A4, transport to the building site;
C4, and module D (A1–A3 + C + D and additional modules: A4 — A5, installation into the building; including provision of all
+ A5 + B6) materials, products and energy, as well as waste processing up
to the end-of waste state or disposal of final residues during the
Production - Module A1-A3 construction process stage.
The product stage includes:
2 Environmental Product Declaration - dormakaba - Automatic Swing Door Operator ED 900
Use stage - Module B6 benefits.
The use stage related to the operation of the building
includes: Geographic Representativeness
— B6, operational energy use Land or region, in which the declared product system is
manufactured, used or handled at the end of the product´s
End-of-life stage– Modules C1-C4 and D lifespan: Global
The end-of-life stage includes:
— C1, de-construction, demolition:
Comparability
— C2, transport to waste processing;
Basically, a comparison or an evaluation of EPD data is only
— C3, waste processing for reuse, recovery and/or recycling;
possible if all the data sets to be compared were created
— C4, disposal; including provision and all transport, provision
according to EN 15804 and the building context, respectively
of all materials, products and related energy and water use.
the product-specific characteristics of performance, are taken
Module D (Benefits and loads beyond the system boundary)
into account. Background database: GaBi, SP40
includes:
— D, recycling potentials, expressed as net impacts and
LCA: Scenarios and additional technical information
Name Value Unit
Characteristic product properties of biogenic carbon
Electricity consumption ED 900 for 1 year 70.42 kWh
Name ValueUnit
Days per year in use 365 days
kg
Biogenic carbon content in product 0.27 On mode per day 1.8 h
C
Idle mode per day 22.2 h
Biogenic carbon content in accompanying kg
packaging 0.41 C On mode power 22.09 W
Idle mode power 6.9 W
End of life (C1-C4)
C1: The product dismantling from the building is done manually
Transport from the gate to the site (A4) without environmental burden.
Name Value Unit C2: Transport to waste management is 50 km.
Litres of fuel (per 1 kg) 0.00276 l/100km Name Value Unit
Capacity utilisation (including empty runs) 55 % Collected separately waste type 12.43 kg
Transport distance via medium truck 100 km Recycling 8.18 kg
Energy recovery 1.89 kg
The product is transported via truck. The product is stored in
the dormakaba logistic center in Germany. The main Landfilling 2.36 kg
distribution region for the ED 900 is North America. In order to The product is disassembled in a recycling process.
allow scaling to a specific point of installation 100 km are Material recycling is then assumed for the metals and
declared. electronics. The plastic components are assumed to be
incinerated with energy recovery. Electromechanics and minor
Installation into the building (A5) proportions of residues arising from the recycling process are
landfilled.
Name Value Unit
Region for the End of Life is: Global.
Waste packaging (paper and plastic) 1,11 kg
Reuse, recovery and/or recycling potentials (D), relevant
Reference service life scenario information
Name Value Unit Name Value Unit
Life Span according to the manufacturer 10 a Recycling 100 %
Collection rate is 100%.
Operational energy use (B6)
The use stage is declared for 10 years
3 Environmental Product Declaration - dormakaba - Automatic Swing Door Operator ED 900
LCA: Results
DESCRIPTION OF THE SYSTEM BOUNDARY (X = INCLUDED IN LCA; MND = MODULE OR INDICATOR NOT DECLARED; MNR
= MODULE NOT RELEVANT)
Benefits and
Construction loads beyond
Product stage Use stage End of life stage
process stage the system
boundaries
la ire ta m w a Ry lp p u s tro p s n a rT g n iru tc a fu n a M e h t m o rf tro p s n a rTe tis e h t o t e ta g y lb m e s s A e s U e c n a n e tn ia M ria p e R tn e m e c a lp e R tn e m h s ib ru fe R y g re n e la n o ita re p Oe s u re ta w la n o ita re p Oe s u n o itc u rts n o c -e Dn o itilo m e d tro p s n a rT g n is s e c o rp e ts a W la s o p s iD -e s u e R-y re v o c e R-g n ilc y c e Rla itn e to p
A1 A2 A3 A4 A5 B1 B2 B3 B4 B5 B6 B7 C1 C2 C3 C4 D
X X X X X MND MND MNR MNR MNR X MND X X X X X
RESULTS OF THE LCA - ENVIRONMENTAL IMPACT according to EN 15804+A2: 1 piece Automatic Swing Door Operator ED
900
Parameter Unit A1-A3 A4 A5 B6 C1 C2 C3 C4 D
GWP-total kg CO 2 eq 5.01E+01 1.18E-01 1.57E+00 2.85E+02 0 6.2E-02 6.22E+00 4.2E-02 -1.39E+01
GWP-fossil kg CO 2 eq 5.27E+01 1.13E-01 3.9E-02 2.83E+02 0 5.9E-02 4.89E+00 4.2E-02 -1.38E+01
GWP-biogenic kg CO 2 eq -2.72E+00 5E-03 1.53E+00 9.45E-01 0 3E-03 1.33E+00 1.43E-04 -3.6E-02
GWP-luluc kg CO 2 eq 6.7E-02 2.69E-06 2.58E-05 4.11E-01 0 1.4E-06 2.88E-04 1.21E-04 -7E-03
ODP kg CFC11 eq 4.49E-09 1.2E-17 2.83E-16 6.24E-12 0 6.22E-18 2.62E-15 1.55E-16 -2.62E-11
AP mol H+ eq 2.14E-01 1.13E-04 4.39E-04 6.26E-01 0 5.89E-05 1E-03 3.01E-04 -5.3E-02
EP-freshwater kg P eq 2.04E-04 2.42E-08 5.53E-08 7.57E-04 0 1.26E-08 4.16E-07 7.2E-08 -2.37E-05
EP-marine kg N eq 3.8E-02 3.61E-05 1.59E-04 1.39E-01 0 1.88E-05 2.58E-04 7.74E-05 -7E-03
EP-terrestrial mol N eq 4E-01 4.01E-04 2E-03 1.46E+00 0 2.09E-04 5E-03 8.5E-04 -7.9E-02
kg NMVOC
POCP 1.19E-01 1.02E-04 4.2E-04 3.81E-01 0 5.3E-05 7.12E-04 2.34E-04 -2.6E-02
eq
ADPE kg Sb eq 1.12E-02 3.4E-09 4.46E-09 8.21E-05 0 1.77E-09 3.63E-08 3.76E-09 -3E-03
ADPF MJ 8.17E+02 1.61E+00 4.95E-01 4.98E+03 0 8.35E-01 2.55E+00 5.5E-01 -1.9E+02
m3 world eq
WDP 9.42E+00 2.22E-04 1.94E-01 6.18E+01 0 1.15E-04 6.37E-01 4E-03 -1.88E+00
deprived
GWP = Global warming potential; ODP = Depletion potential of the stratospheric ozone layer; AP = Acidification potential of land and water; EP =
Eutrophication potential; POCP = Formation potential of tropospheric ozone photochemical oxidants; ADPE = Abiotic depletion potential for non-fossil
resources; ADPF = Abiotic depletion potential for fossil resources; WDP = Water (user) deprivation potential)
RESULTS OF THE LCA - INDICATORS TO DESCRIBE RESOURCE USE according to EN 15804+A2: 1 piece Automatic Swing
Door Operator ED 900
Parameter Unit A1-A3 A4 A5 B6 C1 C2 C3 C4 D
PERE MJ 1.92E+02 5E-03 1.34E+01 2.21E+03 0 3E-03 9.52E+00 7.2E-02 -4.87E+01
PERM MJ 2.22E+01 0 -1.33E+01 0 0 0 -8.88E+00 0 0
PERT MJ 2.14E+02 5E-03 9E-02 2.21E+03 0 3E-03 6.41E-01 7.2E-02 -4.87E+01
PENRE MJ 7.36E+02 1.61E+00 4.95E-01 4.98E+03 0 8.36E-01 8.33E+01 5.5E-01 -1.9E+02
PENRM MJ 8.08E+01 0 0 0 0 0 -8.08E+01 0 0
PENRT MJ 8.17E+02 1.61E+00 4.95E-01 4.98E+03 0 8.36E-01 2.55E+00 5.5E-01 -1.9E+02
SM kg 5.66E+00 0 0 0 0 0 0 0 0
RSF MJ 0 0 0 0 0 0 0 0 0
NRSF MJ 0 0 0 0 0 0 0 0 0
FW m3 3.25E-01 9.08E-06 5E-03 2.55E+00 0 4.72E-06 1.5E-02 1.39E-04 -9.5E-02
PERE = Use of renewable primary energy excluding renewable primary energy resources used as raw materials; PERM = Use of renewable primary
energy resources used as raw materials; PERT = Total use of renewable primary energy resources; PENRE = Use of non-renewable primary energy
excluding non-renewable primary energy resources used as raw materials; PENRM = Use of non-renewable primary energy resources used as raw
materials; PENRT = Total use of non-renewable primary energy resources; SM = Use of secondary material; RSF = Use of renewable secondary fuels;
NRSF = Use of non-renewable secondary fuels; FW = Use of net fresh water
RESULTS OF THE LCA – WASTE CATEGORIES AND OUTPUT FLOWS according to EN 15804+A2:
1 piece Automatic Swing Door Operator ED 900
Parameter Unit A1-A3 A4 A5 B6 C1 C2 C3 C4 D
HWD kg 3.63E-05 1.56E-10 7.3E-10 2.06E-06 0 8.11E-11 8.81E-09 8.39E-09 -3.9E-06
NHWD kg 3.33E+00 1.64E-04 4.9E-02 3.54E+00 0 8.55E-05 5.16E-01 2.77E+00 -6.13E-01
RWD kg 2.8E-02 1.73E-06 2.6E-05 7.56E-01 0 8.97E-07 1E-04 6.26E-06 -1.3E-02
CRU kg 0 0 0 0 0 0 0 0 0
MFR kg 0 0 0 0 0 0 6.55E+00 0 0
MER kg 0 0 0 0 0 0 0 0 0
EEE MJ 0 0 2.37E+00 0 0 0 1.11E+01 0 0
4 Environmental Product Declaration - dormakaba - Automatic Swing Door Operator ED 900
EET MJ 0 0 4.3E+00 0 0 0 2.45E+01 0 0
HWD = Hazardous waste disposed; NHWD = Non-hazardous waste disposed; RWD = Radioactive waste disposed; CRU = Components for re-use;
MFR = Materials for recycling; MER = Materials for energy recovery; EEE = Exported electrical energy; EET = Exported thermal energy
RESULTS OF THE LCA – additional impact categories according to EN 15804+A2-optional:
1 piece Automatic Swing Door Operator ED 900
Parameter Unit A1-A3 A4 A5 B6 C1 C2 C3 C4 D
Disease
PM 2.07E-06 5.96E-10 2.43E-09 5.25E-06 0 3.1E-10 1.2E-08 3.72E-09 -6.78E-07
incidence
IR kBq U235 eq 3.34E+00 2.46E-04 4E-03 1.24E+02 0 1.28E-04 1E-02 6.44E-04 -2.1E+00
ETP-fw CTUe 3.71E+02 1.14E+00 2.35E-01 2.13E+03 0 5.92E-01 9.74E-01 3.14E-01 -6.43E+01
HTP-c CTUh 2.96E-08 2.14E-11 1.24E-11 5.89E-08 0 1.11E-11 8.17E-11 4.66E-11 2.28E-08
HTP-nc CTUh 1.55E-06 9.15E-10 5.38E-10 2.17E-06 0 4.76E-10 7.72E-09 5.13E-09 2.7E-06
SQP SQP 4.67E+02 4E-03 1.31E-01 1.59E+03 0 2E-03 7.57E-01 1.15E-01 -1.51E+01
PM = Potential incidence of disease due to PM emissions; IR = Potential Human exposure efficiency relative to U235; ETP-fw = Potential comparative
Toxic Unit for ecosystems; HTP-c = Potential comparative Toxic Unit for humans (cancerogenic); HTP-nc = Potential comparative Toxic Unit for humans
(not cancerogenic); SQP = Potential soil quality index
Disclaimer 1 – for the indicator “Potential Human exposure efficiency relative to U235”. This impact category deals mainly with the
eventual impact of low-dose ionizing radiation on human health of the nuclear fuel cycle. It does not consider effects due to possible
nuclear accidents, occupational exposure or radioactive waste disposal in underground facilities. Potential ionizing radiation from the
soil, radon and from some construction materials is also not measured by this indicator.
Disclaimer 2 – for the indicators “abiotic depletion potential for non-fossil resources”, “abiotic depletion potential for fossil resources”,
“water (user) deprivation potential, deprivation-weighted water consumption”, “potential comparative toxic unit for ecosystems”,
“potential comparative toxic unit for humans – cancerogenic”, “Potential comparative toxic unit for humans - not cancerogenic”,
“potential soil quality index”. The results of this environmental impact indicator shall be used with care as the uncertainties on these
results are high as there is limited experience with the indicator.
This EPD was created using a software tool.
References
ISO 14025 Council on machinery, and amending Directive 95/16/EC
DIN EN ISO 14025:2011-10, Environmental labels and
declarations — Type III environmental declarations — IBU 2021
Principles and procedures General Instructions for the EPD programme of Institut Bauen
und Umwelt e.V. Version 2.0, Berlin: Institut Bauen und Umwelt
EN 15804 e.V., 2021. www.ibu-epd.com
EN 15804+A2:2019+AC:2021, Sustainability of construction
works — Environmental Product Declarations — Core rules for GaBi
the product category ofconstruction products Sphera Solutions GmbH Gabi Software System and Database
for Life Cycle Engineering 1992-2020 Version 10.0.0.71
EN 18650 University of Stuttgart Leinfelden-Echterdingen
EN 18650-1:2010, Powered pedestrian doors - Part 1: Product
requirements and test methods GaBi ts documentation
GaBi life cycle inventory data documentation
EN 18650 (https://www.gabisoftware.com/support/gabi/gabidatabase-
EN 18650-2:2010, Powered pedestrian doors - Part 2: Safety at 2020-lci-documentation/)
powered pedestrian doors
LCA-tool dormakaba
EN 16005 LCA tool, version ENS (drive system) Tool No.: IBU-DOR-
EN 16005: 2013-01, Power operated pedestrian doorsets - 202108-LT1-EN Developed by Sphera Solutions GmbH
Safety in use - Requirements and test methods
PCR Part A
EN 60335 PCR – Part A: Calculation Rules for the Life Cycle Assessment
EN 60335-1, -2-103:2020-08, Household and similar electrical and Requirements on the Project Re-port according to EN
appliances - Safety - Part 1: General requirements 15804+A2:2019, Version 1.0, Institut Bauen und Umwelt e.V.,
www.ibu-epd.com
EN 61000
EN 61000-1-2:2017-07, Electromagnetic compatibility (EMC) - PCR Part B
Part 1-2: General - Methodology for the achievement of PCR – Part B: Requirements for the EPD for Drive systems for
functional safety of electrical and electronic systems including automatic doors and gates, version 08/2021, Institut Bauen und
equipment with regard to electromagnetic phenomena Umwelt e.V., www.ibu-epd-com.
EN ISO 13849 REACH
EN ISO 13849-1:2021-08, Safety of machinery - Safety-related Registration, Evaluation, Authorisation and Restriction of
parts of control systems - Part 1: General principles for design Chemicals (REACH), Regulation (EC) No 1907/2006
Machinery Directive 2011/65/EU ROHS3 Directive
Directive 2006/42/EC of the European Parliament and of the Directive 2011/65/EU of the European Parliament and of the
5 Environmental Product Declaration - dormakaba - Automatic Swing Door Operator ED 900
Council of 8 June 2011 on the restriction of the use of certain https:echa.europa.eu/de/home
hazardous substances in electrical and electronic equipment
European Chemicals Agency (ECHA)
6 Environmental Product Declaration - dormakaba - Automatic Swing Door Operator ED 900
Publisher
Institut Bauen und Umwelt e.V. +49 (0)30 3087748- 0
Hegelplatz 1 info@ibu-epd.com
10117 Berlin www.ibu-epd.com
Germany
Programme holder
Institut Bauen und Umwelt e.V. +49 (0)30 3087748- 0
Hegelplatz 1 info@ibu-epd.com
10117 Berlin www.ibu-epd.com
Germany
Author of the Life Cycle Assessment
dormakaba International Holding GmbH +49 2333 793-0
DORMA Platz 1 info.de@dormakaba.com
58256 Ennepetal www.dormakaba.com
Germany
Owner of the Declaration
dormakaba International Holding GmbH +49 2333 793-0
DORMA Platz 1 info.de@dormakaba.com
58256 Ennepetal www.dormakaba.com
Germany
7 Environmental Product Declaration - dormakaba - Automatic Swing Door Operator ED 900
