ENVIRONMENTAL PRODUCT DECLARATION
as per ISO 14025 and EN 15804+A2
Owner of the Declaration dormakaba International Holding GmbH
Publisher Institut Bauen und Umwelt e.V. (IBU)
Programme holder Institut Bauen und Umwelt e.V. (IBU)
Declaration number EPD-DOR-20210285-CBA9-EN
Issue date 08.08.2022
Valid to 07.08.2027
Automatic Revolving Door KTV A
Dormakaba
www.ibu-epd.com | https://epd-online.com
General Information
Dormakaba Automatic Revolving Door KTV A
Programme holder Owner of the declaration
IBU – Institut Bauen und Umwelt e.V. dormakaba International Holding GmbH
Hegelplatz 1 DORMA Platz 1
10117 Berlin 58256 Ennepetal
Germany Germany
Declaration number Declared product / declared unit
EPD-DOR-20210285-CBA9-EN The declaration represents one automatic revolving door, consisting of four
(4) door leaves with a diameter of 3000 mm and a height of 2200 mm,
consisting of the following items:
• Drum wall
• Canopy construction
• Door wings
• Turnstile fittings
• KT FLEX Direct drive unit
• Electric accessories / sensors
• Floor ring
• Product Packaging
This declaration is based on the product category rules: Scope:
Automatic doors, automatic gates, and revolving door systems, This EPD is a specific product declaration for the KTV A automatic
01.08.2021 revolving door. The underlying life cycle assessment is based on the entire
(PCR checked and approved by the SVR) life cycle of this specific revolving door. The KTV A is manufactured at the
dormakaba production facility in Sofia, Bulgaria.
Data represents the year 2021.
Issue date The owner of the declaration shall be liable for the underlying information
and evidence; the IBU shall not be liable with respect to manufacturer
08.08.2022
information, life cycle assessment data and evidences.
The EPD was created according to the specifications of EN 15804+A2. In
Valid to
the following, the standard will be simplified as EN 15804.
07.08.2027
Verification
The standard EN 15804 serves as the core PCR
Independent verification of the declaration and data according to ISO
14025:2011
internally X externally
Dipl.-Ing. Hans Peters
(Chairman of Institut Bauen und Umwelt e.V.)
Florian Pronold Dr.-Ing. Wolfram Trinius,
(Managing Director Institut Bauen und Umwelt e.V.) (Independent verifier)
1 Environmental Product Declaration - Dormakaba - Automatic Revolving Door KTV A
Product
• DIN 18650-2: Powered pedestrian doors. Part 2: Safety
Product description/Product definition at powered pedestrian doors.
The KTV revolving door range is designed for installation in Performance data of the product with respect to its
entrance areas where interior environmental control coupled characteristics in accordance with the relevant technical
with elegant aesthetics are desired. dormakaba KTV revolving provision which can be applied are mentioned above.
doors hold back noise, dust and dirt, reliably protect employees
near the entrances from drafts, and help to keep heating cost Application
down. They also allow for a smooth flow of traffic. Automatic revolving doors may be used to provide a
comfortable entry and exit in many applications in the facade of
Revolving doors offer a number of benefits for installers, or within a building. Typical applications include:
architects, specifiers and user among others:
• Office / commercial buildings
• Extensive design flexibility in terms of planning and • Airports
technical requirements • Public buildings
• Visually, technically and economically the ideal • Hospitals
application • Hotels
• Optimization of the building energy balance Automatic revolving doors are used to control the pedestrian
• Efficient noise protection flow in combination with an optimal thermal separation of the
• Tailored integrated application combining industrial inside and outside climates during normal use.
engineering precision and assured quality.
KTV A revolving doors can optionally be equipped with:
For placing the product on the market in the European
• 3- or 4-wing design
Union/European Free Trade Association (EU/EFTA) (with the
• Glazed drum walls or with metal paneling
exception of Switzerland), the following legal provisions apply:
• Additional curved sliding doors in front of the
• 2011/65/EU ROHS3 Directive entrance to act as night shields
as well as the harmonized norms based on these provisions: Observance of the applicable regulations and standards
guarantee the highest level of pedestrian safety.
• DIN EN ISO 13849-1: Safety of machinery - Safety-
related parts of control systems - Part
Technical Data
1: General principles for design.
Performance data of the product according to the harmonized
• DIN EN ISO 12100: Safety of machinery - Basic
norms, based on the harmonization provisions. The following
concepts - Risk assessment and risk reduction.
technical data excluding lighting also apply:
• DIN EN 16005: Power operated pedestrian doorsets -
Safety in use - Requirements and
test methods.
• DIN EN 61000 - 6 - 2: Electromagnetic compatibility
(EMC). Part 6-2: Generic standards: Interference
resistance for industrial environments.
• DIN EN 61000 - 6 - 3: Electromagnetic compatibility
Base materials/Ancillary materials
(EMC). Part 6-3: Generic standards: Emission standard
For the main product components: One automatic revolving
for residential, commercial and light-industrial
door, consisting of four (4) door leaves and with a diameter of
environments.
3000mm and a height of 2200mm, the product composition of
• DIN EN 61000 - 3 - 2: Electromagnetic compatibility-3-2:
the KTV A is as follows:
Limits - Limits for harmonic
current emissions.
• DIN EN 61000 - 3 - 3: Electromagnetic compatibility-3-3:
Limits - Limitation of voltage
changes, voltage fluctuations and flicker in public low-
voltage supply systems.
• DIN EN 55022: Information technology equipment -
Radio disturbance characteristics
- Limits and methods of measurement.
• DIN EN 60335 - 1: Safety of household and similar
electrical appliances. Part 1: General
requirements.
• EN 60335-2-103: Household and similar electrical
appliances. Safety. Particular requirements for drives for
gates, doors and windows.
The KTV A includes partial articles which contain substances
The CE-marking takes into account the proof of conformity with listed in the Candidate List of REACH Regulation
the respective harmonized norms based on the legal provisions 1907/2006/EC (date: 08.07.2021) exceeding 0.1 percentage by
above. For the application and use, the respective national mass: yes
provisions apply. In addition to the harmonized standards, the
• Lead (Pb): 7439-92-1 (CAS-No.) is used in some of the
following national standards have also been applied and
alloys. The concentration of lead in each individual alloy
complied with:
does not exceed 4.0% (by mass).
• DIN 18650-1: Powered pedestrian doors. Part 1: The Candidate List can be found on the ECHA website
Product requirements and test methods. address: https:echa.europa.eu/de/home
2 Environmental Product Declaration - Dormakaba - Automatic Revolving Door KTV A
Reference service life
The reference service life of dormakaba's automatic revolving
doors is about 20 years, depending on the application and
frequency of use. This is consistent with approximately 10
million cycles over the door's service life.
LCA: Calculation rules
— A5, installation into the building; including provision of all
Declared Unit materials, products and energy, as well as waste processing up
The declared unit is 1 piece of the product: 876.16 kg to the end-ofwaste state or disposal of final residues during the
Name Value Unit construction process stage.
Declared unit for revolving door system* 6.6 m2
Use stage - Module B6
Mass of the entire system (excl. packaging) 876 kg
The use stage related to the operation of the buildingincludes:
Conversion factor to 1 kg 876 -
— B6, operational energy use
Grammage of the components 133 kg/m2
Dimensions for revolving door, diameter 3000 mm End-of-life stage– Modules C1-C4 and D
The end-of-life stage includes:
Dimensions for revolving door, height 2200 mm
— C1, de-construction, demolition:
* Area represents the cross-sectional area of the door, which is — C2, transport to waste processing;
designed to fit in an opening of 3000-mm wide — C3, waste processing for reuse, recovery and/orrecycling;
by 2200-mm high. — C4, disposal; including provision and all transport, provision
of all materials, products and related energy and water
use.Module D (Benefits and loads beyond the system
System boundary
boundary) includes:
The type of EPD is: cradle to gate with options, modules C1–
— D, recycling potentials, expressed as net impactsand
C4, and module D (A1–A3 + C + D and additional modules: A4
benefits.
+ A5 + B6)
Geographic Representativeness
Production - Module A1-A3 Land or region, in which the declared product system is
The product stage includes: manufactured, used or handled at the end of the product´s
— A1, raw material extraction, processing and mechanical lifespan: Bulgaria
treatments, processing of secondary material input (e.g.
recycling processes),
— A2, transport to the manufacturer, Comparability
— A3, manufacturing and assemblyincluding provision of all Basically, a comparison or an evaluation of EPD data is only
materials, products and energy, as well as waste processing up possible if all the data sets to be compared were created
to the end-of waste state. according to EN 15804 and the building context, respectively
the product-specific characteristics of performance, are taken
Construction stage - Modules A4-A5 into account. Background database: GaBi ts, SP40.
The construction process stage includes:
— A4, transport to the building site;
LCA: Scenarios and additional technical information
Installation into the building (A5)
Characteristic product properties of biogenic carbon
Name Value Unit
Information on describing the Biogenic Carbon Content at
Waste packaging (paper and plastic) 35.7 kg
factory gate
Name ValueUnit Reference service life
Biogenic carbon content in product 13.55 kg Name Value Unit
C
Life Span according to the manufacturer 20 a
Biogenic carbon content in accompanying kg
12.52
packaging C Operational energy use (B6)
The use stage is declared for 20 years.
The following technical scenario information is required for the Name Value Unit
declared modules Electricity consumption (per year) 177.05 kWh
Transport to the building site (A4) Days per year in use 365 days
Name Value Unit On mode per day 2,5 h
Litres of fuel (per 1 kg) 0.00276 l/100km Idle mode per day 10,5 h
Transport distance 100 km Off mode per day 11 h
Capacity utilisation (including empty runs) 55 % On mode power 31,49 W
Idle mode power 18,9 W
Transport distance is declared for a distance of 100km by truck
in order to allow scaling to a specific point of Off mode power 18,9 W
installation.
3 Environmental Product Declaration - Dormakaba - Automatic Revolving Door KTV A
The product is disassembled in a recycling process. Material
End of life (C1-C4)
recycling is then assumed for the metals, electronic and
C1: The product dismantling from the building is done manually
electromechanics. The plastic components are assumed to be
without environmental burden.
incinerated with energy recovery. Minor proportions of residues
C2: Transport to waste treatment at end of life is 50km.
arising from the recycling process, glass/inert materials are
Name Value Unit landfilled. Region for the End of Life is: Global.
Collected separately waste type waste type 876 kg
Recycling 442 kg Reuse, recovery and/or recycling potentials (D), relevant
scenario information
Energy recovery 13.6 kg
Collection rate is 100%.
Landfilling 420 kg
Transport to waste management 50 km
4 Environmental Product Declaration - Dormakaba - Automatic Revolving Door KTV A
LCA: Results
DESCRIPTION OF THE SYSTEM BOUNDARY (X = INCLUDED IN LCA; MND = MODULE OR INDICATOR NOT DECLARED; MNR
= MODULE NOT RELEVANT)
Benefits and
Construction loads beyond
Product stage Use stage End of life stage
process stage the system
boundaries
la ire ta m w a Ry lp p u s tro p s n a rT g n iru tc a fu n a M e h t m o rf tro p s n a rTe tis e h t o t e ta g y lb m e s s A e s U e c n a n e tn ia M ria p e R tn e m e c a lp e R tn e m h s ib ru fe R y g re n e la n o ita re p Oe s u re ta w la n o ita re p Oe s u n o itc u rts n o c -e Dn o itilo m e d tro p s n a rT g n is s e c o rp e ts a W la s o p s iD -e s u e R-y re v o c e R-g n ilc y c e Rla itn e to p
A1 A2 A3 A4 A5 B1 B2 B3 B4 B5 B6 B7 C1 C2 C3 C4 D
X X X X X MND MND MNR MNR MNR X MND X X X X X
RESULTS OF THE LCA - ENVIRONMENTAL IMPACT according to EN 15804+A2: Automatic Revolving Door KTV A
Parameter Unit A1-A3 A4 A5 B6 C1 C2 C3 C4 D
GWP-total kg CO 2 eq 4.08E+03 7.97E+00 5.25E+01 1.43E+03 0 3.81E+00 8.63E+01 6.42E+00 -2.06E+03
GWP-fossil kg CO 2 eq 4.17E+03 7.62E+00 5.53E+00 1.43E+03 0 3.64E+00 3.54E+01 6.38E+00 -2.05E+03
GWP-biogenic kg CO 2 eq -9.68E+01 3.52E-01 4.7E+01 4.75E+00 0 1.68E-01 5.09E+01 2.18E-02 -4.76E+00
GWP-luluc kg CO 2 eq 2.33E+00 1.81E-04 1.04E-03 2.07E+00 0 8.67E-05 2.45E-03 1.84E-02 -7.08E-01
ODP kg CFC11 eq 7.29E-09 8.05E-16 1.09E-14 3.14E-11 0 3.85E-16 2.37E-14 2.37E-14 -1.39E-08
AP mol H+ eq 2.23E+01 7.63E-03 1.43E-02 3.15E+00 0 3.65E-03 1.36E-02 4.58E-02 -7.87E+00
EP-freshwater kg P eq 4.26E-03 1.63E-06 2.05E-06 4E-03 0 7.8E-07 3.72E-06 1.1E-05 -1.23E-03
EP-marine kg N eq 3.55E+00 2.43E-03 5.05E-03 6.99E-01 0 1.16E-03 3.8E-03 1.18E-02 -1.06E+00
EP-terrestrial mol N eq 3.93E+01 2.7E-02 6.43E-02 7.34E+00 0 1.29E-02 6.3E-02 1.29E-01 -1.15E+01
kg NMVOC
POCP 9.75E+00 6.86E-03 1.34E-02 1.92E+00 0 3.28E-03 1.04E-02 3.57E-02 -3.36E+00
eq
ADPE kg Sb eq 7.73E-02 2.29E-07 1.67E-07 4.13E-04 0 1.09E-07 3.39E-07 5.73E-07 -2.69E-02
ADPF MJ 5.37E+04 1.08E+02 1.72E+01 2.51E+04 0 5.17E+01 2.71E+01 8.37E+01 -2.86E+04
m3 world eq
WDP 1.3E+03 1.49E-02 6.42E+00 3.11E+02 0 7.14E-03 8.87E+00 6.69E-01 -1.77E+02
deprived
GWP = Global warming potential; ODP = Depletion potential of the stratospheric ozone layer; AP = Acidification potential of land and water; EP =
Eutrophication potential; POCP = Formation potential of tropospheric ozone photochemical oxidants; ADPE = Abiotic depletion potential for non-fossil
resources; ADPF = Abiotic depletion potential for fossil resources; WDP = Water (user) deprivation potential)
RESULTS OF THE LCA - INDICATORS TO DESCRIBE RESOURCE USE according to EN 15804+A2: Automatic Revolving Door
KTV A
Parameter Unit A1-A3 A4 A5 B6 C1 C2 C3 C4 D
PERE MJ 1.88E+04 3.41E-01 4.11E+02 1.11E+04 0 1.63E-01 5.17E+02 1.1E+01 -1.25E+04
PERM MJ 9.19E+02 0 -4.08E+02 0 0 0 -5.11E+02 0 0
PERT MJ 1.97E+04 3.41E-01 3.29E+00 1.11E+04 0 1.63E-01 6.24E+00 1.1E+01 -1.25E+04
PENRE MJ 5.32E+04 1.08E+02 9.03E+01 2.51E+04 0 5.17E+01 5.34E+02 8.37E+01 -2.87E+04
PENRM MJ 5.8E+02 0 -7.31E+01 0 0 0 -5.07E+02 0 0
PENRT MJ 5.37E+04 1.08E+02 1.72E+01 2.51E+04 0 5.17E+01 2.71E+01 8.37E+01 -2.87E+04
SM kg 3.69E+01 0 0 0 0 0 0 0 0
RSF MJ 0 0 0 0 0 0 0 0 0
NRSF MJ 0 0 0 0 0 0 0 0 0
FW m3 5.92E+01 6.11E-04 1.51E-01 1.28E+01 0 2.92E-04 2.1E-01 2.11E-02 -2.44E+01
PERE = Use of renewable primary energy excluding renewable primary energy resources used as raw materials; PERM = Use of renewable primary
energy resources used as raw materials; PERT = Total use of renewable primary energy resources; PENRE = Use of non-renewable primary energy
excluding non-renewable primary energy resources used as raw materials; PENRM = Use of non-renewable primary energy resources used as raw
materials; PENRT = Total use of non-renewable primary energy resources; SM = Use of secondary material; RSF = Use of renewable secondary fuels;
NRSF = Use of non-renewable secondary fuels; FW = Use of net fresh water
RESULTS OF THE LCA – WASTE CATEGORIES AND OUTPUT FLOWS according to EN 15804+A2:
Automatic Revolving Door KTV A
Parameter Unit A1-A3 A4 A5 B6 C1 C2 C3 C4 D
HWD kg 1.07E-04 1.05E-08 3.01E-08 1.04E-05 0 5.02E-09 6.89E-08 1.28E-06 -1.31E-04
NHWD kg 8.44E+02 1.11E-02 1.96E+00 1.78E+01 0 5.29E-03 3.96E+00 4.21E+02 -4.74E+02
RWD kg 2.52E+00 1.16E-04 8.74E-04 3.8E+00 0 5.55E-05 1.23E-03 9.53E-04 -2.88E+00
CRU kg 0 0 0 0 0 0 0 0 0
MFR kg 0 0 0 0 0 0 4.09E+02 0 0
MER kg 0 0 0 0 0 0 0 0 0
EEE MJ 5.15E+00 0 8.09E+01 0 0 0 0 0 0
EET MJ 9.34E+00 0 1.51E+02 0 0 0 0 0 0
5 Environmental Product Declaration - Dormakaba - Automatic Revolving Door KTV A
HWD = Hazardous waste disposed; NHWD = Non-hazardous waste disposed; RWD = Radioactive waste disposed; CRU = Components for re-use;
MFR = Materials for recycling; MER = Materials for energy recovery; EEE = Exported electrical energy; EET = Exported thermal energy
RESULTS OF THE LCA – additional impact categories according to EN 15804+A2-optional:
Automatic Revolving Door KTV A
Parameter Unit A1-A3 A4 A5 B6 C1 C2 C3 C4 D
Disease
PM 2.24E-04 4.01E-08 8.46E-08 1.39E-05 0 1.92E-08 1.16E-07 5.66E-07 -1.3E-04
incidence
IR kBq U235 eq 4.7E+02 1.66E-02 1.3E-01 3.28E+02 0 7.93E-03 1.54E-01 9.8E-02 -5.77E+02
ETP-fw CTUe 3.11E+04 7.66E+01 7.98E+00 5.64E+03 0 3.66E+01 1.09E+01 4.78E+01 -1.1E+04
HTP-c CTUh 7.35E-05 1.44E-09 4.47E-10 1.56E-07 0 6.89E-10 8.42E-10 7.09E-09 -6.96E-07
HTP-nc CTUh 5.58E-05 6.16E-08 2.31E-08 5.74E-06 0 2.95E-08 6.4E-08 7.81E-07 4.97E-06
SQP SQP 1.62E+04 2.78E-01 4.64E+00 4.2E+03 0 1.33E-01 7.89E+00 1.74E+01 -1.15E+03
PM = Potential incidence of disease due to PM emissions; IR = Potential Human exposure efficiency relative to U235; ETP-fw = Potential comparative
Toxic Unit for ecosystems; HTP-c = Potential comparative Toxic Unit for humans (cancerogenic); HTP-nc = Potential comparative Toxic Unit for humans
(not cancerogenic); SQP = Potential soil quality index
Disclaimer 1 – for the indicator IRP
This impact category deals mainly with the eventual impact of low dose ionizing radiation on human health of the nuclear fuel cycle. It
does not consider effects due to possible nuclear accidents, occupational exposure nor radioactive waste disposal in underground
facilities.
Potential ionizing radiation from the soil, from radon and from some construction materials is also not measured by this indicator.
Disclaimer 2 – for the indicators ADPE, ADPF, WDP, ETP-fw, HTP-c, HTP-nc, SQP
The results of this environmental impact indicator shall be used with care as the uncertainties on these results are high or as there is
limited experience with the indicator.
References
DIN 18650-1 DIN EN 61000-6-3
DIN 18650-1/: Powered pedestrian doors. Part 1: Product DIN EN 61000-6-3: Electromagnetic compatibility (EMC). Part
requirements and test methods. 6-3: Generic standards: Emission standard for residential,
commercial and light-industrial environments.
DIN 18650-2
DIN 18650-2/: Powered pedestrian doors. Part 2: Safety at DIN EN ISO 9001
powered pedestrian doors DIN EN ISO 9001: Quality management systems.
DIN EN 16005 DIN EN ISO 12100
DIN EN 16005: Power operated pedestrian doorsets - Safety in DIN EN ISO 12100: Safety of machinery - Basic concepts -
use - Requirements and test methods. Risk assessment and risk reduction.
DIN EN 55022 DIN EN ISO 13849-1
DIN EN 55022: Information technology equipment - Radio DIN EN ISO 13849-1: Safety of machinery - Safety-related
disturbance characteristics - Limits and methods of parts of control systems - Part 1: General principles for design.
measurement.
IEC 60335-2-103
DIN EN 60335 IEC 60335-2-103: Household and similar electrical appliances.
DIN EN 60335 - 1: Safety of household and similar electrical Safety. Part 2-103: Particular requirements for drives for gates,
appliances. Part 1: General requirements. doors and windows.
EN 60335-2-103 REACH Regulation
EN 60335-2-103: Household and similar electrical appliances. REACH Regulation (EC) No 1907/2006 of the European
Safety. Particular requirements for drives for gates, doors and Parliament and of the Council on the Registration, Evaluation,
windows. Authorisation and Restriction of Chemicals.
DIN EN 61000-3-2 RoHS 2011/65/EU
DIN EN 61000-3-2: Electromagnetic compatibility-3-2: Limits - RoHS 2011/65/EU, Directive on the restriction of the use of
Limits for harmonic current emissions. certain hazardous substances in electrical and electronic
equipment.
DIN EN 61000-3-3
DIN EN 61000-3-3: Electromagnetic compatibility-3-3: Limits - European Chemicals Agency (ECHA)
Limitation of voltage changes, voltage fluctuations and flicker in https:echa.europa.eu/de/home
public low-voltage supply systems.
Further References
DIN EN 61000-6-2
DIN EN 61000-6-2: Electromagnetic compatibility (EMC). Part IBU 2021
6-2: Generic standards: Interference resistance for industrial General Instructions for the EPD programme of Institut Bauen
environments. und Umwelt e.V. Version 2.0, Berlin: Institut Bauen und Umwelt
e.V., 2021. www.ibu-epd.com
6 Environmental Product Declaration - Dormakaba - Automatic Revolving Door KTV A
GaBi ts software PCR Part A
Sphera Solutions GmbH PCR – Part A: Calculation Rules for the Life Cycle Assessment
Gabi Software System and Database for Life Cycle and Requirements on the Project Re-port according to EN
Engineering 1992-2020 15804+A2:2019, Version 1.0, Institut Bauen und Umwelt e.V.,
Version 10.0.0.71 www.ibu-epd.com.
University of Stuttgart
Leinfelden-Echterdingen PCR Part B
PCR – Part B: Requirements on the EPD for Automatic doors,
GaBi ts documentation automatic gates, and revolving door systems, 08/2021, Institut
GaBi life cycle inventory data documentation Bauen und Umwelt e.V., www.ibu-epd.com
(https://www.gabisoftware. com/support/gabi/gabidatabase-
2020-lci-documentation/).
LCA-tool dormakaba
LCA tool, version 1.0. ENS (doors)
Developed by Sphera Solutions GmbH.
7 Environmental Product Declaration - Dormakaba - Automatic Revolving Door KTV A
Publisher
Institut Bauen und Umwelt e.V. +49 (0)30 3087748- 0
Hegelplatz 1 info@ibu-epd.com
10117 Berlin www.ibu-epd.com
Germany
Programme holder
Institut Bauen und Umwelt e.V. +49 (0)30 3087748- 0
Hegelplatz 1 info@ibu-epd.com
10117 Berlin www.ibu-epd.com
Germany
Author of the Life Cycle Assessment
Sphera Solutions GmbH +49 711 341817-0
Hauptstraße 111- 113 info@sphera.com
70771 Leinfelden-Echterdingen www.sphera.com
Germany
Owner of the Declaration
dormakaba International Holding GmbH +49 2333 793-0
DORMA Platz 1 info.de@dormakaba.com
58256 Ennepetal www.dormakaba.com
Germany
8 Environmental Product Declaration - Dormakaba - Automatic Revolving Door KTV A
