Environmental product declaration
in accordance with ISO 14025 and EN 15804+A2
bARK Timber Façade System (Glazed Module)
Owner of the declaration: Program operator:
Fasadglas Bäcklin AB The Norwegian EPD Foundation
Product: Declaration number:
bARK Timber Façade System (Glazed Module) NEPD-8393-7945-EN
Declared unit: Registration number:
1 pcs NEPD-8393-7945-EN
This declaration is based on Product Category Rules: Issue date:
CEN Standard EN 15804:2012+A2:2019 serves as core 06.12.2024
PCR
Valid to:
The Norwegian EPD Foundation PCR, Part B: Requirements on the EPD for Curtain walling
16.12.2029
EPD software:
LCAno EPD generator ID: 406971
1 / 12
General information
Product Owner of the declaration:
bARK Timber Façade System (Glazed Module) Fasadglas Bäcklin AB
Contact person:
Phone:
e-mail: Nicola.peterson@fasadglas.se
Program operator: Manufacturer:
The Norwegian EPD Foundation Fasadglas Bäcklin AB
Post Box 5250 Majorstuen, 0303 Oslo, Norway P.O. Box 111 87
Phone: +47 977 22 020 SE-161 11 Bromma, Sweden
web: www.epd-norge.no
Declaration number: Place of production:
Fasadglas Bäcklin Produktion AB
NEPD-8393-7945-EN Norra Oskarsgatan 66
SE-577 35 Hultsfred, Sweden
This declaration is based on Product Category Rules: Management system:
CEN Standard EN 15804:2012+A2:2019 serves as core PCR
PCR, Part B: Requirements on the EPD for Curtain walling
Statement of liability: Organisation no:
The owner of the declaration shall be liable for the underlying SE 556325-9547
information and evidence. EPD Norway shall not be liable with respect
to manufacturer information, life cycle assessment data and
evidences.​
Declared unit: Issue date:
1 pcs bARK Timber Façade System (Glazed Module) 06.12.2024
Declared unit with option: Valid to:
A1-A3,A4,A5,C1,C2,C3,C4,D 06.12.2029
Year of study:
2023
Functional unit: Comparability:
1 unit of a bARK Timber Façade System Module (glazed) with a EPD of construction products may not be comparable if they do not
grammage of 49.57 kg/m². The actual reference size of the declared comply with EN 15804 and seen in a building context.
façade module has dimensions of 2535 x 4641 mm.
General information on verification of EPD from EPD tools: Development and verification of EPD:
Independent verification of data, other environmental information The declaration is created using EPD tool lca.tools ver EPD2022.03,
and the declaration according to ISO 14025:2010, § 8.1.3 and § 8.1.4. developed by LCA.no. The EPD tool is integrated in the company's
Verification of each EPD is made according to EPD-Norway’s management system, and has been approved by EPD Norway.
guidelines for verification and approval requiring that tools are i)
integrated into the company's environmental management system, ii) Developer of EPD: Nicola Peterson
the procedures for use of the EPD tool are approved by EPD-Norway,
Reviewer of company-specific input data and EPD:​ Hans Svärd
and iii) the process is reviewed annually by an independent third
party verifier. See Appendix G of EPD-Norway's General Programme
Instructions for further information on EPD tools
Verification of EPD tool: Approved:
Independent third party verification of the EPD tool, background data
and test-EPD in accordance with EPDNorway's procedures and
guidelines for verification and approval of EPD tools.
Håkon Hauan, CEO EPD-Norge
Third party verifier:
Alexander Borg, Asplan Viak AS
(no signature required)
2 / 12
Product
Product description:
bARK Module is a versatile, pre-fabricated façade system made from high-quality Swedish glulam wood, combined with insulating glass and stone
wool insulation. The proportions between glazed and insulated sections is fully customizable to suit design- and project requirements. The bARK
Module system allows for extensive design flexibility, offering options for size, glass configurations, integrated spandrel glass, metal or wood fillers.
As well as various ventilated exterior cladding choices, including wood panels, stone, ceramic or metal elements.
The insulated sections, as detailed in this declaration, are compossed of a vapor barrier on the interior, stone wool insulation and exterior wind
protection. Typically, the glazed areas make up for 40-60% of the module surface. Installation is completed using steel fittings, tailored to the
building's structural needs.
U-values typically range from 0.25- to 0.8 W/m²·K (depending on the ratio between glazed to insulated areas).
Product specification
Materials Value Unit
Insulation 8,69 %
Rubber 0,62 %
Thermowood 0,74 %
Glulam 21,42 %
Glass 62,31 %
Steel 2,08 %
Aluminum 1,9 %
PVC 2,25 %
Technical data:
Test Standard Class
Watertightness EN 12154 RE 750
Wind load EN 13116 2000 Pa
Curtain Walling SS-EN 13830:2015+A1:2020
Air Permeability EN 12152 AE750
Market:
Scandinavia.
Reference service life, product
Only applicable when modules in the use phase is declared (modules B1-B6).
Reference service life, building or construction works
For commercial or industrial buildings, the service life is estimated around 30 to 60 years depending on various factors; such as quality of
construction, usage, maintenance and technological solutions.
LCA: Calculation rules
Declared unit:
1 pcs bARK Timber Façade System (Glazed Module)
Cut-off criteria:
All major raw materials and all the essential energy is included. The production processes for raw materials and energy flows with very small
amounts (less than 1%) are not included. These cut-off criteria do not​ apply for hazardous materials and substances.
Allocation:
The allocation is made in accordance with the provisions of EN 15804. Incoming energy and water and waste production in-house is allocated
equally among all products through mass allocation. Effects of primary production of recycled materials is allocated to the main product in which
the material was used. The recycling process and transportation of the material is allocated to this analysis.
Data quality:
Specific data for the product composition are provided by the manufacturer. The data represent the production of the declared product and were
collected for EPD development in the year of study. Background data is based on EPDs according to EN 15804 and different LCA databases. The
data quality of the raw materials in A1 is presented in the table below.
3 / 12
Materials Source Data quality Year
Glass S-P-00933 EPD 2019
Insulation NEPD-3414-2027-EN EPD 2021
Metal - Aluminium Modified ecoinvent 3.6 Database 2019
Metal - Steel ecoinvent 3.6 Database 2019
Plastic ecoinvent 3.6 Database 2019
Rubber, synthetic ecoinvent 3.6 Database 2019
Database + EPD
Wood Ecoinvent 3.6 2019
(A1 info)
Wood RTS EPD nro: RTS_44_19 EPD 2019
4 / 12
System boundaries (X=included, MND=module not declared, MNR=module not relevant)
Construction Beyond the system
Product stage Use stage End of life stage
installation stage boundaries
A1 A2 A3 A4 A5 B1 B2 B3 B4 B5 B6 B7 C1 C2 C3 C4 D
X X X X X MND MND MND MND MND MND MND X X X X X
System boundary:
Modules A1-A5 are included in the analysis. It includes the extraction and production of raw materials, transportation to the factory, the
production process itself and transportation to market, and installation at construction site.
Additional technical information:
waR slairetam tropsnarT gnirutcafunaM tropsnarT ylbmessA e​sU ecnanetniaM riapeR tnemecalpeR tnemhsibrufeR lanoitarepO ygrene esu lanoitarepO esu retaw -eD noitcurtsnoc noitilomed tropsnarT etsaW gnissecorp lasopsiD -yrevoceR-esueR laitnetop-gnilcyceR
5 / 12
LCA: Scenarios and additional technical information
The following information describe the scenarios in the different modules of the EPD.
Module A4 = Transport from our factory in Hultsfred to the construction site. Generic distance of 280 km.
Module C1 = includes use of energy for de-construction activities for the different material groups used in the system. C1 thus allocates energy
usage to sorting and demolition activities before each material group undergoes its respective waste treatment processes for the year 2021 as
defined by Statistikkbanken (SSB 2021), Table 09781: Treatment of waste from construction, rehabilitation and demolition of buildings (tonnes), by
material, contents, year and treatment.
Module C2 = A default transport distance of 85 km is recommended for the Swedish market.
Modules C3 and C4 = Waste treatment of the product follows the default values provided in Statistikbanken (SSB 2021), Table 09781: Treatment
of waste from construction, rehabilitation and demolition of buildings (tonnes), by material, contents, year and treatment. This table specified how
different types of raw materials used in A1 will likely be treated during the end-of-life of the product. Waste treatments in C3 include material
recycling and incineration with energy recovery and fly ash extraction. Disposal in C4 consist of landfilling of different waste fractions and of ashes.
Module D = The recyclability of metals, plastics, and electronic components allows the producers a credit for the net scrap that is produced at the
end of a product’s life. The benefits from recycling of net scrap are described in formula from EN 15804:2012+A2:2019. Substitution of heat and
electricity generated by the incineration with energy recovery of plastic insulation and other parts is also calculated in module D.
Capacity utilisation Value
Transport from production place to user (A4) Distance (km) Fuel/Energy Consumption Unit
(incl. return) % (Liter/tonne)
Truck, 16-32 tonnes, EURO 6 (km) - Europe 36,7 % 250 0,043 l/tkm 10,75
Assembly (A5) Unit Value
Electricity, Sweden (kWh) kWh/DU 15,00
De-construction demolition (C1) Unit Value
Demolition of glass per kg kg 363,71
Demolition of hazardous waste per kg kg 50,70
Demolition of plastic per kg kg 16,77
Demolition of wood per kg kg 129,31
Demolition of steel per kg kg 12,14
Demolition of aluminium per kg kg 11,08
Capacity utilisation Value
Transport to waste processing (C2) Distance (km) Fuel/Energy Consumption Unit
(incl. return) % (Liter/tonne)
Truck, 16-32 tonnes, EURO 6 (km) - Europe 36,7 % 85 0,043 l/tkm 3,66
Waste processing (C3) Unit Value
Materials to recycling (kg) kg 432,14
Waste treatment per kg Glass, incineration with fly
kg 9,97
ash extraction (kg)
Waste treatment per kg Plastic, Mixture,
kg 4,48
municipal incineration with fly ash extraction (kg)
Waste treatment per kg Wood, from incineration
kg 75,00
(kg)
Disposal (C4) Unit Value
Landfilling of ashes from incineration of Glass,
kg 10,02
process of ashes and residues (kg)
Waste, inert waste, to landfill (kg) - C4 kg 11,42
Waste, hazardous waste, to landfill (kg) kg 50,70
Landfilling of ashes from incineration of Plastics,
Mixture, municipal incineration with fly ash
kg 0,16
extraction, process per kg ashes and residues - C4
(kg)
Landfilling of ashes from incineration of Wood,
kg 0,86
process per kg ashes and residues - C4 (kg)
Benefits and loads beyond the system
Unit Value
boundaries (D)
Substitution of electricity, in Norway (MJ) MJ 59,17
Substitution of thermal energy, district heating, in
MJ 895,19
Norway (MJ)
Substitution of primary glass with net scrap (kg) -
kg 343,89
GLO
Substitution of plastic granulates (kg) - Global kg 10,85
Substitution of wood chips (kg) kg 54,31
Substitution of primary steel with net scrap (kg) kg 12,13
Substitution of primary aluminium with net scrap
kg 11,07
(kg)
6 / 12
LCA: Results
The LCA results are presented below for the declared unit defined on page 2 of the EPD document.
Environmental impact
Indicator Unit A1-A3 A4 A5 C1 C2 C3 C4 D
GWP-total kg CO2 -eq 7,14E+02 2,38E+01 8,24E-01 7,70E-01 8,10E+00 2,22E+02 1,11E+01 -5,01E+02
GWP-fossil kg CO2 -eq 9,10E+02 2,38E+01 7,59E-01 7,70E-01 8,09E+00 1,16E+01 1,10E+01 -4,95E+02
GWP-biogenic kg CO2 -eq -2,00E+02 9,85E-03 1,54E-02 1,44E-04 3,35E-03 2,10E+02 9,69E-03 -3,85E+00
GWP-luluc kg CO2 -eq 2,99E+00 8,47E-03 4,93E-02 6,07E-05 2,88E-03 1,96E-04 9,56E-02 -2,21E+00
ODP kg CFC11 -eq 5,81E-05 5,39E-06 3,72E-07 1,66E-07 1,83E-06 1,03E-07 6,21E-07 -3,78E-01
AP mol H+ -eq 4,77E+00 6,84E-02 4,94E-03 8,05E-03 2,33E-02 1,42E-02 5,23E-02 -4,57E+00
EP-FreshWater kg P -eq 1,52E-02 1,90E-04 5,13E-05 2,80E-06 6,47E-05 1,86E-05 4,85E-04 -1,22E-02
EP-Marine kg N -eq 1,00E+00 1,35E-02 8,42E-04 3,55E-03 4,60E-03 6,78E-03 1,08E-02 -7,15E-01
EP-Terrestial mol N -eq 1,24E+01 1,51E-01 1,11E-02 3,90E-02 5,15E-02 7,16E-02 1,16E-01 -8,59E+00
POCP kg NMVOC -eq 3,01E+00 5,80E-02 2,53E-03 1,07E-02 1,97E-02 1,76E-02 5,56E-02 -2,28E+00
ADP-minerals&metals1 kg Sb-eq 7,20E-02 6,58E-04 3,04E-05 1,18E-06 2,24E-04 5,15E-06 6,53E-05 -3,00E-02
ADP-fossil1 MJ 1,58E+04 3,60E+02 8,90E+01 1,06E+01 1,22E+02 9,17E+00 1,24E+02 -6,00E+03
WDP1 m3 3,14E+05 3,48E+02 9,03E+03 2,25E+00 1,18E+02 2,99E+01 1,09E+02 -6,02E+04
GWP-total = Global Warming Potential total; GWP-fossil = Global Warming Potential fossil fuels; GWP-biogenic = Global Warming Potential biogenic; GWP-luluc =
Global Warming Potential land use and land use change; ODP = Depletion potential of the stratospheric ozone layer; AP = Acidification potential, Accumulated
Exceedance; EP-freshwater = Eutrophication potential, fraction of nutrients reaching freshwater end compartment: EP-marine = Eutrophication potential, fraction of
nutrients reaching marine end compartment; EP-terrestrial = Eutrophication potential, Accumulated Exceedance; POCP = Formation potential of tropospheric ozone;
ADP-minerals&metals = Abiotic depletion potential for non-fossil resources; ADP-fossil = Abiotic depletion for fossil resources potential; WDP = Water (user)
deprivation potential, deprivation-weighted water consumption
"Reading example: 9,0 E-03 = 9,0*10-3 = 0,009"
*INA Indicator Not Assessed
1. The results of this environmental impact indicator shall be used with care as the uncertainties on these results are high or as there is limited experienced with the
indicator
Remarks to environmental impacts
7 / 12
Additional environmental impact indicators
Indicator Unit A1-A3 A4 A5 C1 C2 C3 C4 D
PM Disease incidence 2,71E-05 1,46E-06 3,56E-08 2,13E-07 4,96E-07 1,50E-07 9,55E-07 -4,81E-05
IRP2 kgBq U235 -eq 1,11E+02 1,57E+00 3,05E+00 4,54E-02 5,35E-01 1,91E-02 1,98E-01 -1,55E+01
ETP-fw1 CTUe 7,22E+03 2,67E+02 4,70E+01 5,79E+00 9,07E+01 3,84E+01 3,10E+02 -1,04E+04
HTP-c1 CTUh 7,20E-07 0,00E+00 1,35E-09 0,00E+00 0,00E+00 3,43E-09 4,85E-08 -4,09E-07
HTP-nc1 CTUh 1,02E-05 2,92E-07 3,25E-08 5,25E-09 9,91E-08 1,59E-07 3,42E-07 -4,68E-06
SQP1 dimensionless 1,23E+04 2,52E+02 3,94E+01 1,34E+00 8,56E+01 1,46E+00 3,18E+02 -7,44E+03
PM = Particulate Matter emissions; IRP = Ionizing radiation – human health; ETP-fw = Eco toxicity – freshwater; HTP-c = Human toxicity – cancer effects; HTP-nc =
Human toxicity – non cancer effects; SQP = Potential Soil Quality Index (dimensionless)
"Reading example: 9,0 E-03 = 9,0*10-3 = 0,009"
*INA Indicator Not Assessed
1. The results of this environmental impact indicator shall be used with care as the uncertainties on these results are high or as there is limited experienced with the
indicator
2. This impact category deals mainly with the eventual impact of low dose ionizing radiation on human health of the nuclear fuel cycle. It does not consider effects due
to possible nuclear accidents, occupational exposure nor due to radioactive waste disposal in underground facilities. Potential ionizing radiation from the soil, from
radon and from some construction materials is also not measured by this indicator.
8 / 12
Resource use
Indicator Unit A1-A3 A4 A5 C1 C2 C3 C4 D
PERE MJ 6,82E+03 5,15E+00 4,28E+01 5,73E-02 1,75E+00 3,45E-01 4,19E+01 -2,19E+03
PERM MJ 1,87E+03 0,00E+00 0,00E+00 0,00E+00 0,00E+00 -1,81E+03 0,00E+00 0,00E+00
PERT MJ 8,68E+03 5,15E+00 4,28E+01 5,73E-02 1,75E+00 -1,81E+03 4,19E+01 -2,19E+03
PENRE MJ 1,55E+04 3,60E+02 8,92E+01 1,06E+01 1,22E+02 9,17E+00 1,24E+02 -5,61E+03
PENRM MJ 5,43E+02 0,00E+00 0,00E+00 0,00E+00 0,00E+00 -3,81E+02 0,00E+00 -4,61E+02
PENRT MJ 1,61E+04 3,60E+02 8,92E+01 1,06E+01 1,22E+02 -3,72E+02 1,24E+02 -6,07E+03
SM kg 5,32E+01 0,00E+00 0,00E+00 5,20E-03 0,00E+00 0,00E+00 1,09E+00 -6,77E-02
RSF MJ 1,16E+01 1,84E-01 1,66E-01 1,41E-03 6,27E-02 7,78E-03 9,20E-02 -1,93E-01
NRSF MJ 1,27E+01 6,59E-01 5,24E-01 2,07E-02 2,24E-01 0,00E+00 9,77E+00 -1,25E+01
FW m3 8,96E+00 3,85E-02 9,72E-02 5,45E-04 1,31E-02 2,80E-02 6,95E-02 -5,33E+00
PERE = Use of renewable primary energy excluding renewable primary energy resources used as raw materials; PERM = Use of renewable primary energy resources used
as raw materials; PERT = Total use of renewable primary energy resources; PENRE = Use of non renewable primary energy excluding non-renewable primary energy
resources used as raw materials; PENRM = Use of non renewable primary energy resources used as raw materials; PENRT = Total use of non renewable primary energy
resources; SM = Use of secondary materials; RSF = Use of renewable secondary fuels; NRSF = Use of non-renewable secondary fuels; FW = Net use of fresh water
"Reading example: 9,0 E-03 = 9,0*10-3 = 0,009"
*INA Indicator Not Assessed
9 / 12
End of life - Waste
Indicator Unit A1-A3 A4 A5 C1 C2 C3 C4 D
HWD kg 3,96E+00 1,86E-02 4,65E-03 3,12E-04 6,31E-03 0,00E+00 6,13E+01 -9,89E-01
NHWD kg 1,23E+02 1,75E+01 2,94E-01 1,25E-02 5,95E+00 9,97E+00 1,17E+01 -6,25E+01
RWD kg 5,35E-01 2,45E-03 1,34E-03 7,36E-05 8,34E-04 0,00E+00 1,75E-05 -1,83E-02
HWD = Hazardous waste disposed; NHWD = Non-hazardous waste disposed; RWD = Radioactive waste disposed
"Reading example: 9,0 E-03 = 9,0*10-3 = 0,009"
*INA Indicator Not Assessed
End of life - Output flow
Indicator Unit A1-A3 A4 A5 C1 C2 C3 C4 D
CRU kg 0,00E+00 0,00E+00 0,00E+00 0,00E+00 0,00E+00 0,00E+00 0,00E+00 0,00E+00
MFR kg 7,61E+00 0,00E+00 0,00E+00 5,11E-03 0,00E+00 4,32E+02 0,00E+00 0,00E+00
MER kg 1,82E+01 0,00E+00 0,00E+00 1,58E-05 0,00E+00 8,94E+01 0,00E+00 0,00E+00
EEE MJ 1,20E+01 0,00E+00 0,00E+00 5,43E-05 0,00E+00 5,92E+01 0,00E+00 0,00E+00
EET MJ 1,81E+02 0,00E+00 0,00E+00 8,21E-04 0,00E+00 8,95E+02 0,00E+00 0,00E+00
CRU = Components for re-use; MFR = Materials for recycling; MER = Materials for energy recovery; EEE = Exported energy electrical; EET = Exported energy thermal
"Reading example: 9,0 E-03 = 9,0*10-3 = 0,009"
*INA Indicator Not Assessed
Biogenic Carbon Content
Indicator Unit At the factory gate
Biogenic carbon content in product kg C 5,90E+01
Biogenic carbon content in accompanying packaging kg C 0,00E+00
Note: 1 kg biogenic carbon is equivalent to 44/12 kg CO2
10 / 12
Additional requirements
Greenhouse gas emissions from the use of electricity in the manufacturing phase
National production mix from import, low voltage (production of transmission lines, in addition to direct emissions and losses in grid) of applied
electricity for the manufacturing process (A3).
Electricity mix Source Amount Unit
Electricity, Sweden (kWh) ecoinvent 3.6 54,94 g CO2-eq/kWh
Dangerous substances
The product contains no substances given by the REACH Candidate list.
Indoor environment
Additional Environmental Information
Additional environmental impact indicators required in NPCR Part A for construction products
Indicator Unit A1-A3 A4 A5 C1 C2 C3 C4 D
GWPIOBC kg CO2 -eq 9,17E+02 2,38E+01 8,23E-01 7,70E-01 8,10E+00 1,16E+01 1,12E+01 -5,01E+02
GWP-IOBC: Global warming potential calculated according to the principle of instantaneous oxidation. In order to increase the transparency of biogenic carbon​
contribution to climate impact, the indicator GWP-IOBC is required as it declares climate impacts calculated according to the principle of instantaneous oxidation.​
GWP-IOBC is also referred to as GWP-GHG in context to Swedish public procurement legislation.
11 / 12
Bibliography
ISO 14025:2010 Environmental labels and declarations - Type III environmental declarations - Principles and procedures.
ISO 14044:2006 Environmental management - Life cycle assessment - Requirements and guidelines.
EN 15804:2012+A2:2019 Environmental product declaration - Core rules for the product category of construction products.
ecoinvent v3, Allocation, cut-off by classification, Swiss Centre of Life Cycle Inventories.
Iversen et al., (2021) eEPD v2021.09 Background information for EPD generator tool system verification, LCA.no Report number: 07.21
Babwah and Ruttenborg., (2024) EPD generator for PCR IBU: Part B,
Requirements on the EPD for Curtain walling Background information for EPD generator application and LCA data, LCA.no report number: 01.24.
NPCR Part A: Construction products and services. Ver. 2.0. April 2021, EPD-Norge.
IBU 2023 Part B: Requirements on the EPD for Curtain walling version 8, 2023, IBU – Institut Bauen und Umwelt e.V
Program operator and publisher Phone: +47 977 22 020
The Norwegian EPD Foundation e-mail: post@epd-norge.no
Post Box 5250 Majorstuen, 0303 Oslo, Norway web: www.epd-norge.no
Owner of the declaration: Phone:
Fasadglas Bäcklin AB e-mail: Nicola.peterson@fasadglas.se
P.O. Box 111 87 , SE-161 11 Bromma, Sweden web:
Author of the Life Cycle Assessment Phone: +47 916 50 916
LCA.no AS e-mail: post@lca.no
Dokka 6A, 1671 Kråkerøy, Norway web: www.lca.no
Developer of EPD generator Phone: +47 916 50 916
LCA.no AS e-mail: post@lca.no
Dokka 6A, 1671 Kråkerøy, Norway web: www.lca.no
ECO Platform web: www.eco-platform.org
ECO Portal web: ECO Portal
12 / 12
