ENVIRONMENTAL PRODUCT DECLARATION
as per ISO 14025 and EN 15804+A2
Owner of the Declaration bauforumstahl e.V.
Publisher Institut Bauen und Umwelt e.V. (IBU)
Programme holder Institut Bauen und Umwelt e.V. (IBU)
Declaration number EPD-BFS-20230271-IBG3-EN
Issue date 06.10.2023
Valid to 05.10.2028
Structural Steel: Sections and merchant bars
bauforumstahl e.V.
www.ibu-epd.com | https://epd-online.com
1. General Information
bauforumstahl e.V. Structural Steel: Sections and merchant bars
Programme holder Owner of the declaration
IBU – Institut Bauen und Umwelt e.V. bauforumstahl e.V.
Hegelplatz 1 Sohnstraße 65
10117 Berlin 40237 Düsseldorf
Germany Germany
Declaration number Declared product / declared unit
EPD-BFS-20230271-IBG3-EN 1 metric ton of structural steel sections and merchant bars
This declaration is based on the product category rules: Scope:
Structural steels, 01.08.2021 This environmental product declaration (EPD) covers structural steel
(PCR checked and approved by the SVR) sections and merchant bars that are 100 % recycled from steel scrap.
The Life Cycle Assessment refers to an average product and is based on
data collected from the following electric arc furnace plants of
Issue date bauforumstahl e.V. member companies:
06.10.2023
- ArcelorMittal on the sites Differdange/Esch-Belval/Rodange
(Luxembourg), Olaberria/Bergara (Spain), Hunedoara (Romania)
Valid to
- Peiner Träger (Germany)
05.10.2028
- Stahlwerk Thüringen (Germany)
The data used represent >95 % of the annual production of sections and
merchant bars from bauforumstahl e.V. member companies.
The owner of the declaration shall be liable for the underlying information
and evidence; the IBU shall not be liable with respect to manufacturer
information, life cycle assessment data and evidences.
The EPD was created according to the specifications of EN 15804+A2. In
the following, the standard will be simplified as EN 15804.
Verification
Dipl.-Ing. Hans Peters
(Chairman of Institut Bauen und Umwelt e.V.) The standard EN 15804 serves as the core PCR
Independent verification of the declaration and data according to ISO
14025:2011
internally X externally
Florian Pronold Dr.-Ing. Nikolay Minkov,
(Managing Director Institut Bauen und Umwelt e.V.) (Independent verifier)
1 Environmental Product Declaration - bauforumstahl e.V. - Structural Steel: Sections and merchant bars
2. Product
2.1 Product description/Product definition The product for authorization contains substances on the
This EPD applies to structural steel sections and merchant bars ECHA list of substances of very high concern (SVHC) (14
that are 100 % recycled from scrap. It covers steel products of July2021) above 0.1 % by mass: No.
grades S235 to S500. For the placing on the market of the
product in the European Union/European Free Trade The product contains further carcinogenic, mutagenic,
Association (EU/EFTA) (with the exception of Switzerland) reprotoxic (CMR) substances of category 1A or 1B that not in
Regulation (EU) No. 305/2011 (CPR) applies. The product the candidate list, above 0.1 mass % in at least one
needs a Declaration of Performance taking into consideration subproduct: No.
EN 10025-1:2004 Hot rolled products of structural steels – Part
1: General technical delivery conditions and the CE-marking. Biocides have been added to the construction product, or the
For the application and use the respective national provisions product has been treated with biocides (a treated product
apply. pursuant to the Biocidal Product Regulation (EU) No.528/2012):
No.
2.2 Application
Structural steels are intended for bolted, welded or otherwise 2.6 Manufacture
connected constructions of buildings, bridges and other In the electric steel production route scrap is molten in an
structures, or in composite steel and concrete structures. electric arc furnace to obtain
Examples are: liquid steel.
• single-storey buildings (industrial and storage halls, etc.) Refining (lowering of sulphur, phosphorous and other tramp
• multi-storey buildings (offices, residential buildings, elements) and alloying (e.g. about 1 % Mn, 0.2 % Si) and/or
shops, car parks, high rise, etc.) micro-alloying (e.g. about 0.01 % V) is applied to give the
• bridges (railway bridge, road bridge, pedestrian bridge, requested characteristics to the steel.
etc.) At the end of the steelmaking process, the liquid steel is
• other structures (power plants, stadiums, convention transformed into a semi-finished product in a continuous
centres, airports, stations, etc.) casting machine, or in special cases, poured into ingot moulds
to form blocks.
2.3 Technical Data The semi-product (beam-blank, slab, bloom or billet) is hot-
This EPD is valid for sections and merchant bars of varied rolled into the final product dimensions (H-shape, I-shape, U-
grades and different forms of delivery. Specific information on shape, L-shape and other merchant bars).
dimension tolerances, constructional data as well as
mechanical and chemical properties can be found in the Quality control: ISO 9001 Monitoring according to the product
relevant literature and/or the standards. standards, e.g. EN 10025, Part 1.
Constructional data 2.7 Environment and health during manufacturing
Name Value Unit No measures relating to safety, health and environment
Density 7850 kg/m3 protecting during the manufacturing process extending beyond
Modulus of elasticity 210000 N/mm2 national guidelines are required.
Coefficient of thermal expansion 12 10-6K-1 2.8 Product processing/Installation
Thermal conductivity at 20°C λ 48 W/(mK) Processing recommendations:
Melting point depending on the alloy
proportions up to 1536 °C Planning, processing, implementation and intended use of
section and merchant bar constructions have to be carried out
Shear modulus 81000 N/mm2
depending on the respective applications according to the
Performance data of the product is in accordance with the generally recognized rules of engineering and manufacturer's
declaration of performance with respect to its essential recommendations.
characteristics according to EN 10025, Hot rolled products of The standards of EN 1993 and EN 1994 (EUROCODE EC3
structural steels. Further product standards are e.g.: ASTMA36, and EC4) apply to the design of steel
A572, A588, A709, A913/A913M and A992. structures and composite steel and concrete structures. They
include the requirements regarding serviceability, bearing
2.4 Delivery status
capacity, durability and fire resistance of steel structures EC3
The dimensions of the declared products may vary according to and composite steel and concrete structures EC4.
the intended application. The Standard Parts 1+2 of EN 1090 apply to the execution of
steel structures and include the requirements for factory
2.5 Base materials/Ancillary materials
production control.
Structural steels are non-or low-alloy steel products whose
In addition, the European Standards will work in connection
carbon content is between 0 and 0.6 %. Iron is the main
with national amendments, national instructions, guidelines and
component of structural steel. The content of other elements is
publications, as well as legal provisions.
less than 2 %. The exact chemical composition varies
Regarding transport and storage of sections and merchant
depending on the steel grade.
bars, the generally accepted requirements for securing loads
have to be observed.
Auxiliary materials:
Instruction details of the manufacturer based on verified
For the production by electric arc furnace: lime aluminium,
standards and guidelines regarding welding, galvanizing as well
ferroalloys (ferro silicon, ferro manganese, ferro nickel, ferro
as hot and cold forming are to be observed in every case.
niobium, ferro vanadium, ferro titanium)
The rates of these additives depend on the steel grade.
Occupational safety / Environmental protection:
2 Environmental Product Declaration - bauforumstahl e.V. - Structural Steel: Sections and merchant bars
When processing/using structural steel pursuant to the Water
generally recognized rules of engineering there are no Steel is stable to water, insoluble and does not emit substances
measures to be taken which are going beyond the public in water. In case of flooding, no impacts are to be expected.
occupational health and safety. Steel can corrode in the presence of oxygen in the water (=
The processing/using of steel sections and merchant bars does slow oxidation).
not release substantial environmental pollutants. Particular
measures to protect the environment are not required. Mechanical destruction
Due to the ductility of steel, steel structures react resilient in the
Residual material: event of unforeseeable mechanical destruction: In case of a
During processing residual pieces as well as turnings are tensile load necking will occur before cracking. In case of
separately collected. This scrap steel is entirely recycled by lasting high compression load, components of steel may buckle
melting and producing new steel products. or bulge. No splintering or breaking edges shall result.
2.9 Packaging 2.14 Re-use phase
Structural steel is delivered unpacked. General:
After the service life of structural steel constructions, the
2.10 Condition of use material is collected as secondary material for recycling or
Structural steels are non- /low-alloyed steel products generated reuse.
by alloying iron with other metals and non-metals (esp. carbon).
Iron is the main component of steel sections and merchant Recycling:
bars. The components are listed under chapter 2.5 'Base Structural steel is 100 % recyclable to new products of similar
materials'. During usage, no changes in material composition or higher quality. Due to the magnetic properties, even small
shall occur. amounts are regained after dismantling. Possible coatings
(metallic, organic or intumescent) do not limit the recyclability.
2.11 Environment and health during use
On the European market 88 % of the products are used for
The intended use of structural steel does not pose a hazard to closed-loop recycling.
health or the environment in any known way.
Reuse:
2.12 Reference service life
Structural steel elements can be reused. On the European
The reference service life is not relevant for consideration of the
market, 11 % of the products are reused after dismantling.
LCA. As construction products with many different applications,
Data from industry estimates based on the following source:
a reference service life for structural steel as sections and
European Commission Technical Steel Research
merchant bars is not declared here. The purpose, possible
corrosion protection and adequate maintenance are decisive 2.15 Disposal
for service life. Due to its high value, steel scrap is not disposed, but fed into a
well-established endless cycle of reuse and recycling. However,
in case of dumping due to collection loss no environmental
impacts are expected.
2.13 Extraordinary effects
Waste code according to European Waste Catalogue EWC: 17
Fire
04 05 - iron and steel
The material is class A1, i.e. not flammable per EN 13501.
The material does not emit fumes or fire-gases. 2.16 Further information
Name Value Additional information on constructing with steel can be
Building material class acc. /EN 13501-1/ A1 obtained from www.bauforumstahl.de.
3. LCA: Calculation rules
Type of the EPD: cradle-to-gate - with options: Modules A1-A3,
3.1 Declared Unit Modules C1-C4 and Module D were considered.
The reference unit is 1 ton of structural steel - sections and
merchant bars. Modules A1-A3 cover the production stage including the
upstream burdens of purchased raw materials (ferroalloys, lime,
Foreground data describing the on-site production are dolomite, etc.), their transports and the manufacturing at the
integrated into the LCA FE Software model for all sites under production sites under study. Material and energy flows for the
study. The LCI is assessed based on annual production data. electric arc furnace and the hot strip mills are considered.
Background data are taken from the LCA FE Database. Electricity consumption is modelled via residual grid mix (e.g.
Declared unit production in Germany + imports - exports -certified "green"
electricity).
Name Value Unit
Declared unit 1 t
Modules C1-C4 consider the dismantling of the considered
Density 7850 kg/m3 product (C1), the transportation of the dismantled components
Conversion factor to 1 kg 0.001 - to their final EoL destination (C2), the waste processing for
reuse, recovery or recycling (C3) as well as the disposal (C4).
The average EPD is calculated considering a production
volume weighted approach and is representative for all steel
Module D refers to the End-of-Life, including recycling and/or
products covered by the declared unit.
reuse.
3.2 System boundary
3.3 Estimates and assumptions
3 Environmental Product Declaration - bauforumstahl e.V. - Structural Steel: Sections and merchant bars
All assumptions are documented in detail and represent the considered to be good.
reality best possible based on available data.
Due to lack of available datasets for some alloying elements Temporal: All primary data are collected for a representative
(e.g. ferro vanadium) South-African datasets were used instead year. All secondary data come from the Sphera LCA FE
of local data. The use of South-African data sets represents a Databases and are representative of the years 2017-2022. As
'worst case' assumption for European production so the set-up the study intended to compare the product systems for the
scenario is considered conservative approach. reference year 2018-2020, temporal representativeness is
Based on the LCA practitioner's knowledge working with the good.
respective industries, the proxy for silico-manganese was
considered as 75 % ferro manganese and 25 % ferro silicon. 3.7 Period under review
All sites are calculated considering the country-specific residual The foreground data collected by the manufacturer are based
grid mix. on yearly production amounts and refer to the years 2018-
2020.
3.4 Cut-off criteria
No cut-off criteria are applied in this study. All reported data 3.8 Geographic Representativeness
were incorporated and modelled using the best available LCI Land or region, in which the declared product system is
data. manufactured, used or handled at the end of the product´s
Packaging materials and their transportation, or the steel straps lifespan: Western Europe
used to bundle the considered steel products for delivery, are
neglected due to low contribution to the overall life cycle
3.9 Allocation
results.
Primary data are allocated using the partitioning approach
3.5 Background data developed by worldsteel/EUROFER for calculating life cycle
Secondary data from the LCA FE Database (former GaBi) were inventories of co-products in steel production. The so-called co-
used to model the background system in the LCA model. product methodology allocates environmental effects to
the steelmaking process and the emerging co-products (here:
3.6 Data quality EAF slag) based on physical relations. Material-inherent
Technological: All primary and secondary data are modelled to flow properties are thus taken into account.
be specific to the technologies or technology mixes under
3.10 Comparability
study. Where technology-specific data are unavailable, proxy
data are used. The overall technological representativeness is Basically, a comparison or an evaluation of EPD data is only
considered to be good. possible if all the data sets to be compared were created
according to EN 15804 and the building context, respectively
Geographical: All primary and secondary data are collected the product-specific characteristics of performance, are taken
specific to the country / region under study. Where into account. The LCA FE Database (CUP version 2022.2) was
country/region-specific data are unavailable, proxy data are used to calculate the LCA. .
used. The overall geographical representativeness is
4. LCA: Scenarios and additional technical information
Name Value Unit
Characteristic product properties of biogenic carbon
Landfilling - Scenario 1 0 kg
The declared product does not include biogenic carbon.
Landfilling - Scenario 2 0 kg
Note: 1 kg of biogenic carbon is equivalent to 44/12 kg of CO .
2
Landfilling - Scenario 3 10 kg
Re-use, recovery- and recycling potential (D)
End-of-Life Scenarios
The EPD covers three End-of-Life scenarios Name Value Unit
(SteelConstruction-info; European Commission Technical Steel Recycling - Scenario 1 1000 kg
Research): Recycling - Scenario 2 0 kg
• Scenario 1: 100 % Recycling Recycling - Scenario 3 880 kg
• Scenario 2: 100 % Reuse Reuse - Scenario 1 0 kg
• Scenario 3: European average 88 % Recycling, 11 %
Reuse - Scenario 2 1000 kg
Reuse and 1 % Loss
Reuse - Scenario 3 110 kg
End of life (C1-C4)
4 Environmental Product Declaration - bauforumstahl e.V. - Structural Steel: Sections and merchant bars
5. LCA: Results
The following table contains the LCA results for a declared unit of 1 ton structural steel - sections and merchant bars.
DESCRIPTION OF THE SYSTEM BOUNDARY (X = INCLUDED IN LCA; MND = MODULE OR INDICATOR NOT DECLARED; MNR
= MODULE NOT RELEVANT)
Benefits and
Construction loads beyond
Product stage Use stage End of life stage
process stage the system
boundaries
la ire ta m w a Ry lp p u s tro p s n a rT g n iru tc a fu n a M e h t m o rf tro p s n a rTe tis e h t o t e ta g y lb m e s s A e s U e c n a n e tn ia M ria p e R tn e m e c a lp e R tn e m h s ib ru fe R y g re n e la n o ita re p Oe s u re ta w la n o ita re p Oe s u n o itc u rts n o c -e Dn o itilo m e d tro p s n a rT g n is s e c o rp e ts a W la s o p s iD -e s u e R-y re v o c e R-g n ilc y c e Rla itn e to p
A1 A2 A3 A4 A5 B1 B2 B3 B4 B5 B6 B7 C1 C2 C3 C4 D
X X X MND MND MND MND MNR MNR MNR MND MND X X X X X
RESULTS OF THE LCA - ENVIRONMENTAL IMPACT according to EN 15804+A2: 1 ton structural steel sections and merchant
bars
Parameter Unit A1-A3 C1 C2 C3/1 C3/2 C3/3 C4/1 C4/2 C4/3 D/1 D/2 D/3
GWP-total kg CO 2 eq 5.6E+02 2.19E+00 2.51E+00 0 0 0 0 0 1.45E-01 2.85E+02 -5.57E+02 2.1E+02
GWP-fossil kg CO 2 eq 5.6E+02 2.86E+00 2.52E+00 0 0 0 0 0 1.49E-01 2.85E+02 -5.57E+02 2.1E+02
GWP-
biogenic kg CO 2 eq 3.8E-01 -7.61E-01 -2.47E-02 0 0 0 0 0 -4.42E-03 -1.46E-01 -4.09E-01 -1.83E-01
GWP-luluc kg CO 2 eq 6.64E-02 9.32E-02 1.7E-02 0 0 0 0 0 2.75E-04 5.88E-03 -4.66E-02 4.71E-04
kg CFC11
ODP 1.85E-09 5.72E-12 2.48E-13 0 0 0 0 0 3.51E-13 6.23E-13 -1.85E-09 -2.03E-10
eq
AP mol H+ eq 1.4E+00 1.1E-02 2.65E-03 0 0 0 0 0 1.06E-03 6.12E-01 -1.4E+00 4.28E-01
EP-
kg P eq 1.2E-04 5.1E-05 9.03E-06 0 0 0 0 0 2.53E-07 5.17E-05 -1.09E-04 3.72E-05
freshwater
EP-marine kg N eq 3.22E-01 2.17E-03 8.17E-04 0 0 0 0 0 2.71E-04 1.08E-01 -3.21E-01 6.71E-02
EP-terrestrial mol N eq 3.5E+00 2.83E-02 9.87E-03 0 0 0 0 0 2.97E-03 9.45E-01 -3.49E+00 5.15E-01
kg NMVOC
POCP 9.71E-01 8.5E-03 2.25E-03 0 0 0 0 0 8.22E-04 4.37E-01 -9.69E-01 3.09E-01
eq
ADPE kg Sb eq 1.08E-04 1.52E-06 2.55E-07 0 0 0 0 0 1.53E-08 7.1E-04 -1.07E-04 6.64E-04
ADPF MJ 9.01E+03 2.4E+02 3.32E+01 0 0 0 0 0 1.95E+00 2.62E+03 -8.97E+03 1.5E+03
m3 world eq
WDP 5.66E+01 2.3E-01 2.83E-02 0 0 0 0 0 1.64E-02 5.3E+01 -5.66E+01 4.41E+01
deprived
GWP = Global warming potential; ODP = Depletion potential of the stratospheric ozone layer; AP = Acidification potential of land and water; EP =
Eutrophication potential; POCP = Formation potential of tropospheric ozone photochemical oxidants; ADPE = Abiotic depletion potential for non-fossil
resources; ADPF = Abiotic depletion potential for fossil resources; WDP = Water (user) deprivation potential)
RESULTS OF THE LCA - INDICATORS TO DESCRIBE RESOURCE USE according to EN 15804+A2: 1 ton structural steel
sections and merchant bars
Parameter Unit A1-A3 C1 C2 C3/1 C3/2 C3/3 C4/1 C4/2 C4/3 D/1 D/2 D/3
PERE MJ 7.66E+02 1.6E+01 2.3E+00 0 0 0 0 0 2.93E-01 -1.65E+02 -7.64E+02 -2.41E+02
PERM MJ 0 0 0 0 0 0 0 0 0 0 0 0
PERT MJ 7.66E+02 1.6E+01 2.3E+00 0 0 0 0 0 2.93E-01 -1.65E+02 -7.64E+02 -2.41E+02
PENRE MJ 9.02E+03 2.41E+02 3.33E+01 0 0 0 0 0 1.96E+00 2.62E+03 -8.98E+03 1.5E+03
PENRM MJ 0 0 0 0 0 0 0 0 0 0 0 0
PENRT MJ 9.02E+03 2.41E+02 3.33E+01 0 0 0 0 0 1.96E+00 2.62E+03 -8.98E+03 1.5E+03
SM kg 1.16E+03 0 0 0 0 0 0 0 0 -1.65E+02 0 -1.56E+02
RSF MJ 0 0 0 0 0 0 0 0 0 0 0 0
NRSF MJ 0 0 0 0 0 0 0 0 0 0 0 0
FW m3 2.41E+00 1.76E-02 2.66E-03 0 0 0 0 0 4.97E-04 1.2E+00 -2.41E+00 8.72E-01
PERE = Use of renewable primary energy excluding renewable primary energy resources used as raw materials; PERM = Use of renewable primary
energy resources used as raw materials; PERT = Total use of renewable primary energy resources; PENRE = Use of non-renewable primary energy
excluding non-renewable primary energy resources used as raw materials; PENRM = Use of non-renewable primary energy resources used as raw
materials; PENRT = Total use of non-renewable primary energy resources; SM = Use of secondary material; RSF = Use of renewable secondary fuels;
NRSF = Use of non-renewable secondary fuels; FW = Use of net fresh water
RESULTS OF THE LCA – WASTE CATEGORIES AND OUTPUT FLOWS according to EN 15804+A2:
1 ton structural steel sections and merchant bars
Parameter Unit A1-A3 C1 C2 C3/1 C3/2 C3/3 C4/1 C4/2 C4/3 D/1 D/2 D/3
HWD kg 8.39E-07 1.62E-09 1.76E-10 0 0 0 0 0 1E-10 2.02E-08 -8.39E-07 -7.31E-08
NHWD kg 2.9E+00 3.75E-02 5.43E-03 0 0 0 0 0 1E+01 -3.97E+01 -2.9E+00 -3.81E+01
RWD kg 1.05E+00 1.21E-03 6.18E-05 0 0 0 0 0 2.17E-05 -3.26E-04 -1.05E+00 -1.16E-01
CRU kg 0 0 0 0 1E+03 1.1E+02 0 0 0 0 0 0
5 Environmental Product Declaration - bauforumstahl e.V. - Structural Steel: Sections and merchant bars
MFR kg 0 0 0 1E+03 0 8.8E+02 0 0 0 0 0 0
MER kg 0 0 0 0 0 0 0 0 0 0 0 0
EEE MJ 0 0 0 0 0 0 0 0 0 0 0 0
EET MJ 0 0 0 0 0 0 0 0 0 0 0 0
HWD = Hazardous waste disposed; NHWD = Non-hazardous waste disposed; RWD = Radioactive waste disposed; CRU = Components for re-use;
MFR = Materials for recycling; MER = Materials for energy recovery; EEE = Exported electrical energy; EET = Exported thermal energy
RESULTS OF THE LCA – additional impact categories according to EN 15804+A2-optional:
1 ton structural steel sections and merchant bars
Parameter Unit A1-A3 C1 C2 C3/1 C3/2 C3/3 C4/1 C4/2 C4/3 D/1 D/2 D/3
Disease
PM ND ND ND ND ND ND ND ND ND ND ND ND
incidence
kBq U235
IR ND ND ND ND ND ND ND ND ND ND ND ND
eq
ETP-fw CTUe ND ND ND ND ND ND ND ND ND ND ND ND
HTP-c CTUh ND ND ND ND ND ND ND ND ND ND ND ND
HTP-nc CTUh ND ND ND ND ND ND ND ND ND ND ND ND
SQP SQP ND ND ND ND ND ND ND ND ND ND ND ND
PM = Potential incidence of disease due to PM emissions; IR = Potential Human exposure efficiency relative to U235; ETP-fw = Potential comparative
Toxic Unit for ecosystems; HTP-c = Potential comparative Toxic Unit for humans (cancerogenic); HTP-nc = Potential comparative Toxic Unit for humans
(not cancerogenic); SQP = Potential soil quality index
The additional and optional impact categories according to EN15804+A2 are not declared as this is not required according to PCR Part
A.
Disclaimer 1 – for the indicator IRP
This impact category deals mainly with the eventual impact of low-dose ionizing radiation on human health of the nuclear fuel cycle. It
does not consider effects due to possible nuclear accidents, occupational exposure or radioactive waste disposal in underground
facilities. Potential ionizing radiation from the soil, radon and some construction materials is also not measured by this indicator.
Disclaimer 2 – for the indicators ADPE, ADPF, WDP, ETP-fw, HTP-c, HTP-nc, SQP
The results of this environmental impact indicator shall be used with care as the uncertainties on these results are high as there is
limited experience with the indicator.
6. LCA: Interpretation
The following figure shows the results of the individual modules
for all considered End-of-Life scenarios using the example of
climate change.
(module A1-3) dominates the product system for all scenarios.
It is visible that module D varies significantly depending on the
considered End-of-Life scenario. The manufacturing phase The following tables give a detailed evaluation of all LCIA
6 Environmental Product Declaration - bauforumstahl e.V. - Structural Steel: Sections and merchant bars
results of the production phase (A1-A3):
the generation of electricity. Resource Use (fossils) is
Climate Change, Acidification Potential, Eutrophication dominated by the generation of electricity.
Potential (marine, terrestrial) and Photochemical Ozone Total use of renewable and non-renewable primary energy
Creation Potential are mostly caused by onsite emissions, carrier (PERT and PENRT) is dominated by the supply chains
extraction and processing of raw materials as well as the supply of electricity and natural gas.
chain of electricity. Radioactive waste comes from the supply chain of electricity.
Eutrophication Potential (freshwater) is driven by the extraction Non-hazardous wastes is mostly caused during the production
and processing of raw materials as well as the supply chains of of alloying materials. Hazardous waste for deposition is mainly
electricity and natural gas. Ozone Depletion is dominated by produced during generation of natural gas and electricity.
the generation of electricity.
Resource Use (mineral and metals) relates to the use of non-
renewable elements in the production of alloying materials and
7. Requisite evidence
This EPD covers semi-finished structural steel of hot rolled of the surrounding atmosphere (corrosivity categories according
construction products. Further processing and fabrication to EN ISO 12944-2.
depend on the intended application. Therefore, further If required, the surfaces of fabricated structural components are
documentation is not applicable. 7.1 Weathering performance usually protected with anticorrosion material in order to prevent
The rusting rate of unalloyed steel depends on the position of any direct contact with the atmosphere. The weathering of this
the component and the conditions protection depends on the applied protection system.
8. References
CPR "Instrumente zur Wiederverwendung von Bauteilen und
Regulation (EU) No 305/2011 of the European Parliament and hochwertigen Verwertung von Baustoffen"
of the Council of 9 March 2011 laying down harmonised
conditions for the marketing of construction products and LCA FE Software / Database
repealing Council Directive 89/106/EEC Text with EEA LCA for Experts Software System and Database for Life Cycle
relevance Engineering, Sphera Solution GmbH, Leinfelden-Echterdingen,
CUP Version 2022.2 (https://www.gabi-
European Commission Technical Steel Research software.com/support/gabi)
Sansom, M. and Meijer, J.: Life-cycle assessment (LCA) for
steel construction, European Commission technical steel PCR, Part A
research, 2001-12 Product Category Rules for Building-Related Products and
Services, Calculation Rules for the Life Cycle Assessment and
EWC Requirements on the Project Report. Institut Bauen und Umwelt
European Waste Catalogue e.V. (IBU), 2021, www.bau-umwelt.de
German Ministry of Environmental Affairs PCR, Part B
7 Environmental Product Declaration - bauforumstahl e.V. - Structural Steel: Sections and merchant bars
Requirements on the EPD for Structural steels – Institut Bauen Standard specification for high-strength low-alloy steel shapes
und Umwelt e.V., Königswinter (pub.): From the range of of structural quality, produced by quenching and self-tempering
Environmental Product Declarations of Institute Construction process (QST)
and Environment e.V. (IBU), 01/08/2021 (PCR checked and
approved by the SVR) ASTM A992-11(15)
Standard specification for structural steel shapes
SteelConstruction-info
https://www.steelconstruction.info/The_recycling_and_reuse_survey ASTM A1066-11(15)
Standard Specification for High-Strength Low-Alloy Structural
worldsteel/EUROFER Steel Plate Produced by Thermo-Mechanical Controlled
Bollen, J., Avery N., Millar, I. and Broadbent, C.: Methodology to Process (TMCP)
determine the LCI of steel industry co-products, 2013
Standards AWS D1.1/D1.1M-15
Structural Welding Code – Steel
AISC 303-10
Code of Standard Practice for Steel Buildings and Bridges ISO 9001:2015
Quality management systems - Requirements
ANSI/AISC 360-16
Specification for Structural Steel Buildings EN 1090:2018
Execution of steel structures and aluminium structures
ASTM A36-14
Standard specification for carbon structural steel EN 10025:2005
Hot rolled products of structural steels
ASTM A283-18
Standard Specification for Low and Intermediate Tensile ISO 12944-2:2017-11
Strength Carbon Steel Plates Paints and varnishes - Corrosion protection of steel structures
by protective paint systems - Part 2: Classification of
ASTM A514-14 environments
Standard Specification for High-Yield-Strength, Quenched and
Tempered Alloy Steel Plate, Suitable for Welding EN 13501:2010-1
Fire classification of construction products and building
ASTM A572-15 elements
Standard Specification for High-Strength Low-Alloy Columbium-
Vanadium Structural Steel ISO 14001:2015
Environmental management systems - Requirements with
ASTM A573-13 guidance for use
Standard Specification for Structural Carbon Steel Plates of
Improved Toughness ISO 14025
Environmental labels and declarations — Type III
ASTM A588-15 environmental declarations —Principles and procedures
Standard Specification for High-Strength Low-Alloy Structural
Steel, up to 50 ksi [345 MPa] Minimum Yield Point, with EN 1993:2010-12/ Eurocode 3
Atmospheric Corrosion Resistance Design of steel structures
ASTM A633-18 EN 1994:2010-12 / Eurocode 4
Standard Specification for Normalized High-Strength Low-Alloy Design of composite steel and concrete structures
Structural Steel Plates
EN 15804
ASTM A709-13 EN 15804:2019+A2, Sustainability of construction works —
Standard Specification for Structural Steel for Bridges Environmental Product Declarations — Core rules for the
product category of construction products
ASTM A913-15
8 Environmental Product Declaration - bauforumstahl e.V. - Structural Steel: Sections and merchant bars
Publisher
Institut Bauen und Umwelt e.V. +49 (0)30 3087748- 0
Hegelplatz 1 info@ibu-epd.com
10117 Berlin www.ibu-epd.com
Germany
Programme holder
Institut Bauen und Umwelt e.V. +49 (0)30 3087748- 0
Hegelplatz 1 info@ibu-epd.com
10117 Berlin www.ibu-epd.com
Germany
Author of the Life Cycle Assessment
Sphera Solutions GmbH +49 (0)711 341817-0
Hauptstraße 111- 113 info@sphera.com
70771 Leinfelden-Echterdingen www.sphera.com
Germany
Owner of the Declaration
bauforumstahl e.V. 0211-54012080
Sohnstraße 65 zentrale@bauforumstahl.de
40237 Düsseldorf www.bauforumstahl.de
Germany
Stahlwerk Thüringen +49 3671 4550 0
Kronacher Straße 6 info@stahlwerk-thueringen.de
07333 Unterwellenborn www.stahlwerk-thueringen.de
Germany
ArcelorMittal Europe – Long Products – Sections +352 5313 3010
Rue de Luxembourg 66 sections.sales@arcelormittal.com
4221 Esch-sur-Alzette sections.arcelormittal.com
Luxembourg
Peiner Träger GmbH +49 51 71 91-01
Gerhard-Lucas-Meyer-Str. 10 peiner.traeger@salzgitter-ag.de
31226 Peine www.peiner-traeger.de
Germany
9 Environmental Product Declaration - bauforumstahl e.V. - Structural Steel: Sections and merchant bars
