ENVIRONMENTAL PRODUCT DECLARATION
as per ISO 14025 and EN 15804+A2
Owner of the Declaration ARGE – The European Federation of Locks and Building Hardware Manufacturers
Publisher Institut Bauen und Umwelt e.V. (IBU)
Programme holder Institut Bauen und Umwelt e.V. (IBU)
Declaration number EPD-ARG-20230548-IBG1-EN
Issue date 02.04.2024
Valid to 01.04.2029
Glass door hardware
ARGE – The European Federation of Locks
and Building Hardware Manufacturers
This EPD is valid only for products supplied by an ARGE EPD licence holder.
www.ibu-epd.com | https://epd-online.com
1. General Information
ARGE – The European Federation of Locks Glass door hardware
and Building Hardware Manufacturers
Programme holder Owner of the declaration
IBU – Institut Bauen und Umwelt e.V. ARGE – The European Federation of Locks and Building Hardware
Hegelplatz 1 Manufacturers
10117 Berlin Offerstraße 12
Germany 42551 Velbert
Germany
Declaration number Declared product / declared unit
EPD-ARG-20230548-IBG1-EN 1 kg of glass door hardware
This declaration is based on the product category rules: Scope:
Building Hardware products, 01.08.2021 This ARGE EPD covers glass door mechanisms used to support glass
(PCR checked and approved by the SVR) doors and allow their opening and closing by means of a sliding action.
The reference product used to calculate the impact this product group has
on the environment is a mechanism composed of aluminium, steel and
Issue date Zamak. It is the only one assessed for this EPD and serves as a reference
to cover all products within this family. This product has been determined
02.04.2024
in accordance with ARGE and its market share as being the most
representative product of the family.
The owner of the declaration shall be liable for the underlying information
Valid to
and evidence; the IBU shall not be liable with respect to manufacturer
01.04.2029 information, life cycle assessment data and evidences.
The EPD was created according to the specifications of EN 15804+A2. In
the following, the standard will be simplified as EN 15804.
Verification
The standard EN 15804 serves as the core PCR
Independent verification of the declaration and data according to ISO
14025:2011
internally X externally
Dipl.-Ing. Hans Peters
(Chairman of Institut Bauen und Umwelt e.V.)
Florian Pronold Dr. Matthew Fishwick,
(Managing Director Institut Bauen und Umwelt e.V.) (Independent verifier)
1 Environmental Product Declaration - ARGE – The European Federation of Locks and Building Hardware Manufacturers - Glass door hardware
2. Product
made of Zamak are die-cast.
2.1 Product description/Product definition
This EPD covers glass door hardware used to support glass Stainless steel is produced by combining iron with chromium
doors and allow their opening and closing. as well as other elements depending on the desired
For the application and use the respective national provisions characteristics. Components made of steel are formed by
at the place of use apply. stamping or other types of mechanical processing.
2.2 Application
Acetal, or polyoxymethylene (POM), is produced by
These products are designed to be integrated into door polymerisation of anhydrous formaldehyde. Components made
assemblies made of glass. Their purpose is to ensure the of Acetal are formed by injection moulding or other thermal
opening and closing of a door. They may be used for either forming processes.
interior or exterior doors in accordance with manufacturer's
instructions.
PP (polypropylene) is a thermoplastic polymer produced from
propylene by a polymerisation process. Components made of
2.3 Technical Data
PP are formed by injection moulding or other thermal forming
Ideally, products should comply with a suitable technical
processes.
specification. EN 1527:2019+A1:2021, Building hardware –
Hardware for sliding doors and folding doors – Requirements
PVC (polyvinyl chloride) is a thermoplastic polymer produced
and test methods is an example of such a specification and
via polymerisation of vinyl chloride. Components made of PVC
some products will comply with this. The relevant grading
are formed by injection moulding or other thermal forming
structure is shown in the following table:
processes.
Name Value Unit
Category of door 1 - 3 PEHD (polyethylene high-density) is a thermoplastic polymer
Door mass 1 - 4 produced from the monomer ethylene. Components made of
Size of Test Panel Used 0 - 4 PEHD are formed by injection moulding or other thermal
forming processes.
Corrosion resistance 0 - 5
Slam test resistance 1 - 3
1) This product/article/at least one partial article contains
Horizontal static load test resistance 1 - 3 substances listed in the ECHA candidate list (date: 14.06.2023)
Static load test resistance 0, 1 exceeding 0.1 percentage by mass: Certain components may
Initial friction maximum permitted value 1 - 3 contain small amounts of lead (CAS no. 7439-92-1) as an
alloying element.
Durability 1 - 6
2) This product/article/at least one partial article contains other
2.4 Delivery status
cancerogenic, mutagenic, reprotoxic (CMR) substances in
The products are sold by unit. Deliveries of individual items are categories 1A or 1B which are not on the ECHA candidate list,
possible but are an exception. Standard deliveries comprise a exceeding 0.1 percentage by mass: no.
larger quantity of glass door hardware as it is marketed as
"B2B" product and not to end-users. 3) Biocide products were added to this construction product or it
has been treated with biocide products (this then concerns a
2.5 Base materials/Ancillary materials
treated product as defined by the (EU) Ordinance on Biocide
Composition of product analysed for this EPD:
Products No. 528/2012): no.
The values given in the table below are for the product 2.6 Manufacture
analysed for this EPD: Manufacture of glass door hardware normally follows a 3-step
Name Value Unit procedure:
Aluminium 79.13 % 1. Manufacture of the components: this step may include
Steel 12.38 % surface treatment in the factory or by external
Zamak 5.71 % contractors.
2. Pre-assembly of modules (in the factory).
Stainless steel 1.99 %
3. Final assembly (in the factory).
Acetal 0.41 %
PP (polypropylene) 0.37 % 2.7 Environment and health during manufacturing
PVC (polyvinyl chloride) 0.00463 % Regular measurements of air quality and noise levels are
carried out by the manufacturers, the ARGE member
PEHD (polyethylene high-density) 0.00139 %
companies. The results shall be within the mandatory safety
Aluminium is a non-ferrous metal produced from bauxite by levels. In areas where employees are exposed to chemical
the Bayer process. Components made of aluminium are products, the required protective clothing and technical
manufactured by extrusion or other types of mechanical protective devices shall be provided. Regular health checks are
processing. mandatory for employees in production facilities.
Steel is produced by combining iron with carbon as well as 2.8 Product processing/Installation
other elements depending on the desired characteristics. The installation of the product may vary depending on the type
Components made of steel are formed by stamping or other of door and the specific situation, but the products shall not
types of mechanical processing. require energy consumption for installation.
Zamak is an alloy with a base metal of zinc and alloying 2.9 Packaging
elements of aluminium, magnesium, and copper. Components
2 Environmental Product Declaration - ARGE – The European Federation of Locks and Building Hardware Manufacturers - Glass door hardware
Normally, each individual product is packed in paper or Fire
cardboard. These individual products are then packed in a There are no specific fire resistance requirements.
cardboard box and stacked on wooden pallets for transport to
the customer. Water
The declared product is intended to be used in buildings under
Waste from product packaging is collected separately for waste normal conditions (indoor or outdoor use). It shall not emit
disposal (including recycling). hazardous substances in the event of flooding.
2.10 Condition of use
Mechanical destruction
Once installed, the products shall require no servicing during Mechanical destruction of the declared product shall not
their expected service lives. There shall be no consumption of materially alter its composition or have any adverse effect on
water or energy linked to their use, and they shall not cause the environment.
any emissions.
2.14 Re-use phase
2.11 Environment and health during use
Removal of glass door hardware (for re-use or recycling) shall
No environmental damage or health risks are to be expected have no adverse effect on the environment.
during normal conditions of use.
2.15 Disposal
2.12 Reference service life
Glass door hardware should be re-cycled wherever possible,
The reference service life is 30 years under normal working providing that there is no adverse effect on the environment.
conditions. This corresponds to passing a mechanical The waste code in accordance with the European Waste Code
endurance test of 100.000 cycles as specified in the EN 1527. is 17 04 07.
The reference service life is dependent on the actual frequency
of use and environmental conditions. It is required that 2.16 Further information
installation, as well as maintenance of the product, must be Details of all types and variants can be found on the
done in line with instructions provided by the manufacturer. manufacturers' websites. The respective website addresses are
available at https://arge.org.
2.13 Extraordinary effects
3. LCA: Calculation rules
according to European averages, with the remaining waste
3.1 Declared Unit divided between incineration and landfill. Such a mixed
The declared unit for all products covered by ARGE EPD is 1 scenario is declared due to the complex material mix of the
kg (of product). Since individual products will rarely weigh product and the dependency of the EoL-route on the EoL-route
exactly 1 kg it is necessary to establish the exact weight of the of the product the glass door hardware has been integrated
product and then use this as a correction factor to determine into.
the true values for 1 kg of product in the tables (Section 5). In practice, the end of life has been modelled as follows:
Declared unit • when a material is sent for recycling, generic transport
Name Value Unit and electric consumption of a shredder is taken into
account (corresponding to the process 'Grinding,
Declared unit 1 kg
metals'). Only then, is the material considered to have
Mass of declared product 4.32 kg
attained the 'end-of-waste' state.
Raw density 1 kg/m3 • each type of waste is modelled as a transport to the
treatment site with a distance of 30 km. Parts sent for
recycling include electricity consumption (grinding) and
3.2 System boundary a flow ('Materials for recycling, unspecified').
Type of the EPD: "cradle to gate with options, with modules C1
3.3 Estimates and assumptions
– C4, and module D (A1-A3, C1-C3, D and additional
modules)" The LCA data of the declared product had been calculated from
the production data of one ARGE member company. This
The analysis of the product life cycle includes the production company had been chosen by ARGE as being representative
and transport of the raw materials, the manufacture of the by virtue of its production processes and market share. The
product and the packaging materials which are declared in chosen product follows the "worst-case" principle as explained
modules A1-A3. in Section 6 - LCA interpretation.
Losses during production are considered as waste and are sent
3.4 Cut-off criteria
for recycling. No recycling processes are taken into account
The cut-off criteria considered are 1% of renewable and non-
except for transport and electricity consumption for grinding the
renewable primary energy usage and 1% of the total mass of
metals. When recycled metals are used as raw material only
that unit process. The total neglected input flows per module
their transformation process is taken into account and not the
shall be at a maximum of 5% of energy usage and mass.
extraction of the raw material.
A4 module represents the transport of the finished glass door
For this study, all input and output flows have been considered
gear to the installation site.
at 100%, including raw materials as per the product
There is no waste associated with the installation of the
composition provided by the manufacturer and packaging of
product. The A5 module therefore represents only the disposal
raw materials as well as the final product. Energy and water
of the product packaging.
consumption have also been considered at 100% according to
The End-of-Life (EoL) stages are also considered. The
the data provided.
transportation to the EoL disposal site is taken into account in
module C2. Module C4 covers the disposal of the locks.
With the approach chosen, no significant environmental
Module C3 covers the recycling of the individual elements
3 Environmental Product Declaration - ARGE – The European Federation of Locks and Building Hardware Manufacturers - Glass door hardware
impacts are known to have been cut off. In this EPD, a representative product has been selected to
represent the product group, considering the most common
3.5 Background data material types of the products covered in this product group.
For the life cycle modelling of the considered product, all
relevant background datasets are taken from ecoinvent v3.8 3.7 Period under review
(system model: cut-off by classification). The data of the LCA is based on the annual production data of
an ARGE member from 2013, considered also representative
3.6 Data quality for the year 2022.
The objective of this evaluation is to evaluate the environmental
impacts generated by the products throughout their entire life 3.8 Geographic Representativeness
cycles. To this end, ISO 14040, ISO 14044 and EN 15804 have Land or region, in which the declared product system is
been met regarding the quality of data on the following different manufactured, used or handled at the end of the product´s
criteria: lifespan: Europe
Time: The life cycle inventory data used come from:
3.9 Allocation
• Data collected specifically for this study on the ARGE
The product assessed for the calculation of this EPD is
member company's manufacturing site. Datasets are
produced by one manufacturer on one site. All data were
based on 1-year averaged data (time period: January
provided by this manufacturer of the products by unit, and then
2013 to December 2013 considered representative for
divided by the mass of the product to give a value per kg of
2022).
product produced.
• In the absence of collected data, generic data from the
ecoinvent v3.8 database have
The assumptions relating to the EoL of the product are
been used. This is updated regularly and is
described in the section System Boundaries.
representative of current processes (the entire database
having been updated in 2021). 3.10 Comparability
Geography: Data on the composition of products, process
Basically, a comparison or an evaluation of EPD data is only
technologies, wastage, etc. come from production site of the
possible if all the data sets to be compared were created
ARGE member company. Generic data on processing
according to EN 15804 and the building context, respectively
processes come from the ecoinvent database, representative
the product-specific characteristics of performance, are taken
for European production processes.
into account.
Technology: Material shaping technologies are based on
ecoinvent v3.8 (system model: cut-off by classification) has
European technology in the case of the use of generic data.
been used as the background database.
4. LCA: Scenarios and additional technical information
End of life (C1-C4)
Characteristic product properties of biogenic carbon
Note: 1 kg of biogenic carbon is equivalent to 44/12 kg of CO . Name Value Unit
2
Collected separately waste type 1 kg
Information on the biogenic carbon content at factory gate
Recycling 0.513 kg
Name Value Unit
Energy recovery 0.224 kg
kg
Biogenic carbon content in product 0 Landfilling 0.263 kg
C
Biogenic carbon content in accompanying kg It is assumed that a 16-32-ton truck is used to transport the
0.0354
packaging C product:
- Transport to shredding facility for metal recovery: 150 km
- Transport to municipal waste incineration plant: 50 km
The following information is the basis of the declared modules
- Transport to landfill: 30 km
within the LCA in this EPD.
Transport to the building site (A4) Reuse, recovery and/or recycling potentials (D), relevant
Name Value Unit scenario information
Litres of fuel 25.8 l/100km
Module D contains the benefits and loads beyond the system
Transport distance 3500 km
boundary related to the recycling of metals, which result from
Capacity utilisation (including empty runs) 36 % the treatment of recycled materials from the point of end-of-
waste status to the point of substitution (as costs) and the
Installation into the building (A5)
substitution of primary resources (as benefits).
Name Value Unit
Material loss 0.088 kg According to EN 16710, clause 6.4.3.3: 'In module D
substitution effects are calculated only for the resulting net
output flow.
Reference service life
Name Value Unit For building hardware, the following rules apply for the
quantification of net output flows:
Reference service life (condition of use: see
30 a - all production scrap and cuttings leave modules A1-B3 as
§2.13)
sorted scrap without allocated burdens from primary production;
Test cycles over RSL (EN 1527) 100'000 cycles
the corresponding amounts are declared as material for
recycling (MFR);
4 Environmental Product Declaration - ARGE – The European Federation of Locks and Building Hardware Manufacturers - Glass door hardware
- net amounts of a metal leaving the product system are
quantified as the material for recycling leaving modules A1-C4 Negative net output flows have been considered in the
minus the input of secondary scrap (secondary material, SM) to quantification of module D.
the product system;
- in the case of brass and zinc alloys, which are composed of It also includes the benefits and loads related to 'exported
two different constituting metals, no difference shall be made energy electricity' and 'exported energy heat' resulting from the
between the input of secondary constituting metals (Cu and Zn; energy recovery from plastic wastes in a municipal waste
Cu and Sn) and its alloys (CuZn; CuSn). incineration plant as modelled in Modules A3, A5 and C4.
5 Environmental Product Declaration - ARGE – The European Federation of Locks and Building Hardware Manufacturers - Glass door hardware
5. LCA: Results
In Table 1 "Description of the system boundary", the declared modules are indicated with an "X"; all modules that are not declared
within the EPD but where additional data are available are indicated with "MND". Those data can also be used for building assessment
scenarios. The values are declared with three valid digits in exponential form.
The set of characterisation factors EF3.0 has been used for the life cycle assessment.
DESCRIPTION OF THE SYSTEM BOUNDARY (X = INCLUDED IN LCA; MND = MODULE OR INDICATOR NOT DECLARED; MNR
= MODULE NOT RELEVANT)
Benefits and
Construction loads beyond
Product stage Use stage End of life stage
process stage the system
boundaries
la ire wta am R y lp p u s tro p s n a rT g n iru tc a fu n a M tro p s nm ae o rh r
T
f te tis e h t o t e ta g y lb m e s s A e s U e c n a n e tn ia M ria p e R tn e m e c a lp e R tn e m h s ib ru fe R la n o ity ag rr ee pn Oe e s u la n o ita r re et pa Ow e s u n o itc u rts n eo Dc -n o itilo m e d tro p s n a rT g n is s ee tsc ao Wrp la s o p s iD e s u e R- y re v o c e R- g n ilc y c e R- la itn e to p
A1 A2 A3 A4 A5 B1 B2 B3 B4 B5 B6 B7 C1 C2 C3 C4 D
X X X X X MND MND MNR MNR MNR MND MND X X X X X
RESULTS OF THE LCA - ENVIRONMENTAL IMPACT according to EN 15804+A2: 1 kg of glass door gear
Parameter Unit A1-A3 A4 A5 C1 C2 C3 C4 D
GWP-total kg CO2 eq 1.65E+01 6.52E-01 2.32E-01 0 1.67E-02 3.78E-03 1.44E-02 -7.72E+00
GWP-fossil kg CO2 eq 1.66E+01 6.52E-01 2.33E-02 0 1.67E-02 3.77E-03 1.44E-02 -7.69E+00
GWP-biogenic kg CO2 eq -2.09E-01 0 2.09E-01 0 0 0 0 0
GWP-luluc kg CO2 eq 4.53E-02 2.61E-04 1.24E-06 0 6.69E-06 9.41E-06 3.03E-06 -2.84E-02
ODP kg CFC11 eq 6.44E-07 1.51E-07 6.91E-10 0 3.88E-09 1.91E-10 1.4E-09 -2.57E-07
AP mol H+ eq 1.12E-01 1.85E-03 1.72E-05 0 4.75E-05 1.94E-05 3.92E-05 -5.03E-02
EP-freshwater kg P eq 5.56E-04 4.65E-06 2.96E-08 0 1.19E-07 4.24E-07 7.41E-08 -2.82E-04
EP-marine kg N eq 1.73E-02 3.68E-04 6.11E-06 0 9.44E-06 2.49E-06 1.42E-05 -7.46E-03
EP-terrestrial mol N eq 1.91E-01 4.1E-03 6.6E-05 0 1.05E-04 2.88E-05 1.55E-04 -8.21E-02
kg NMVOC
POCP 5.51E-02 1.58E-03 1.85E-05 0 4.04E-05 7.88E-06 4.56E-05 -2.45E-02
eq
ADPE kg Sb eq 2.07E-04 2.31E-06 1.14E-08 0 5.93E-08 9.14E-09 2.34E-08 1.54E-05
ADPF MJ 1.59E+02 9.89E+00 4.76E-02 0 2.54E-01 7.99E-02 1.11E-01 -6.94E+01
m3 world eq
WDP 2.51E+00 3.01E-02 3E-04 0 7.72E-04 8.93E-04 -1.21E-03 -1.07E+00
deprived
GWP = Global warming potential; ODP = Depletion potential of the stratospheric ozone layer; AP = Acidification potential of land and water; EP =
Eutrophication potential; POCP = Formation potential of tropospheric ozone photochemical oxidants; ADPE = Abiotic depletion potential for non-fossil
resources; ADPF = Abiotic depletion potential for fossil resources; WDP = Water (user) deprivation potential)
RESULTS OF THE LCA - INDICATORS TO DESCRIBE RESOURCE USE according to EN 15804+A2: 1 kg of glass door gear
Parameter Unit A1-A3 A4 A5 C1 C2 C3 C4 D
PERE MJ 1.68E+01 1.39E-01 -7.08E-01 0 3.56E-03 1.52E-02 1.13E-02 -9.25E+00
PERM MJ 1.78E+00 0 -2.15E-01 0 0 0 0 0
PERT MJ 1.86E+01 1.39E-01 -9.23E-01 0 3.56E-03 1.52E-02 1.13E-02 -9.25E+00
PENRE MJ 1.58E+02 9.89E+00 3.38E-01 0 2.54E-01 8.07E-02 2.18E-01 -6.95E+01
PENRM MJ 4.61E-01 0 -2.9E-01 0 0 0 -1.07E-01 0
PENRT MJ 1.59E+02 9.89E+00 4.76E-02 0 2.54E-01 8.07E-02 1.11E-01 -6.95E+01
SM kg 4.24E-01 0 0 0 0 0 0 0
RSF MJ 0 0 0 0 0 0 0 0
NRSF MJ 0 0 0 0 0 0 0 0
FW m3 1.03E-01 1.05E-03 5.19E-05 0 2.69E-05 5.15E-05 2.06E-04 -5.16E-02
PERE = Use of renewable primary energy excluding renewable primary energy resources used as raw materials; PERM = Use of renewable primary
energy resources used as raw materials; PERT = Total use of renewable primary energy resources; PENRE = Use of non-renewable primary energy
excluding non-renewable primary energy resources used as raw materials; PENRM = Use of non-renewable primary energy resources used as raw
materials; PENRT = Total use of non-renewable primary energy resources; SM = Use of secondary material; RSF = Use of renewable secondary fuels;
NRSF = Use of non-renewable secondary fuels; FW = Use of net fresh water
RESULTS OF THE LCA – WASTE CATEGORIES AND OUTPUT FLOWS according to EN 15804+A2:
1 kg of glass door gear
Parameter Unit A1-A3 A4 A5 C1 C2 C3 C4 D
HWD kg 1.39E-03 2.58E-05 2.15E-07 0 6.62E-07 2.84E-08 1.84E-07 9.86E-04
NHWD kg 4.68E+00 5.2E-01 3.19E-03 0 1.33E-02 3.01E-04 3.42E-01 -1.9E+00
RWD kg 5.39E-04 1.43E-04 6.17E-07 0 3.67E-06 1.08E-06 1.47E-06 -2.13E-04
CRU kg 0 0 0 0 0 0 0 0
MFR kg 3.21E-01 0 9.3E-02 0 0 5.65E-01 0 0
MER kg 0 0 0 0 0 0 0 0
6 Environmental Product Declaration - ARGE – The European Federation of Locks and Building Hardware Manufacturers - Glass door hardware
EEE MJ 2.63E-03 0 3.71E-02 0 0 0 4.55E-03 0
EET MJ 1.74E-02 0 2.45E-01 0 0 0 3.01E-02 0
HWD = Hazardous waste disposed; NHWD = Non-hazardous waste disposed; RWD = Radioactive waste disposed; CRU = Components for re-use;
MFR = Materials for recycling; MER = Materials for energy recovery; EEE = Exported electrical energy; EET = Exported thermal energy
RESULTS OF THE LCA – additional impact categories according to EN 15804+A2-optional:
1 kg of glass door gear
Parameter Unit A1-A3 A4 A5 C1 C2 C3 C4 D
Disease
PM 1.38E-06 5.24E-08 3E-10 0 1.34E-09 5.19E-11 1.03E-09 -6.49E-07
incidence
IR kBq U235 eq 2.31E-01 4.29E-02 1.88E-04 0 1.1E-03 7.28E-04 5.85E-04 -8.02E-02
ETP-fw CTUe 4.73E+02 7.76E+00 4.49E-02 0 1.99E-01 4.02E-02 1.14E+02 -1.68E+02
HTP-c CTUh 2.65E-08 2.5E-10 3.37E-12 0 6.4E-12 1.08E-12 1.19E-11 -8.83E-09
HTP-nc CTUh 4.88E-07 7.84E-09 1.37E-10 0 2.01E-10 3.49E-11 1.95E-10 -1.47E-07
SQP SQP 5.25E+01 6.89E+00 3.03E-02 0 1.77E-01 1.23E-02 1.99E-01 -1.1E+01
PM = Potential incidence of disease due to PM emissions; IR = Potential Human exposure efficiency relative to U235; ETP-fw = Potential comparative
Toxic Unit for ecosystems; HTP-c = Potential comparative Toxic Unit for humans (cancerogenic); HTP-nc = Potential comparative Toxic Unit for humans
(not cancerogenic); SQP = Potential soil quality index
Disclaimer 1 – for the indicator 'Potential Human exposure efficiency relative to U235'. This impact category deals mainly with the
eventual impact of low-dose ionizing radiation on human health of the nuclear fuel cycle. It does not consider effects due to possible
nuclear accidents, occupational exposure or radioactive waste disposal in underground facilities. Potential ionizing radiation from the
soil, radon and from some construction materials is also not measured by this indicator.
Disclaimer 2 – for the indicators 'abiotic depletion potential for non-fossil resources', 'abiotic depletion potential for fossil resources',
'water (user) deprivation potential, deprivation-weighted water consumption', 'potential comparative toxic unit for ecosystems', 'potential
comparative toxic unit for humans – cancerogenic', 'Potential comparative toxic unit for humans - not cancerogenic', 'potential soil
quality index'. The results of this environmental impact indicator shall be used with care as the uncertainties on these results are high
as there is limited experience with the indicator.
6. LCA: Interpretation
7 Environmental Product Declaration - ARGE – The European Federation of Locks and Building Hardware Manufacturers - Glass door hardware
Figure 1 illustrates the relative contributions of the different modules along the life cycle of the declared products.
are in the order of 25 % to 30 % of the impacts over the product
Figure 1: Environmental impacts of glass door hardware life cycle (modules A1-A3) and relate basically to the recycling
along its life cycle of metals; module. Only for ADP elements, the negative net
amount of zinc leaving the product system leads to additional
The largest part of environmental impacts is caused during burdens in module D from the compensation of material losses
production (modules A1-A3); comparably small impacts are with primary production of zinc.
caused during the transport of the product to the construction In this EPD, a representative product has been selected to
site (via the manufacturer of the product, which the glass door represent the product group, considering the most common
gear has been integrated into). materialisation of the products covered in this product group.
This has been done based on the knowledge of ARGE
All the other modules related to the product life cycle are not members on the composition of the declared products. In in-
significant. depth analysis of variability has not been conducted for this
product group.
Benefits and burdens beyond the system boundary (module D)
7. Requisite evidence
No testing results are required by the PCR part B.
8. References
Product category rules of IBU rules for the product category of construction products.
IBU (2021) EN 17610
IBU (2021): General Instructions for the EPD Programme of the EN 17610:2022, Building hardware - Environmental product
Institut Bauen und Umwelt e.V. (General Instructions for the declarations - Product category rules complementary to EN
IBU EPD Programme). Version 2.0, Institut Bauen und Umwelt, 15804 for building hardware.
Berlin.
ISO 14025
IBU (2021) ISO 14025:2006-07, Environmental labels and declarations -
IBU (2021): PCR Part A: Calculation rules for the life cycle Type III Environmental declarations - Principles and
assessment and requirements on the project report according procedures.
to EN 15804+A2. Version 1.3., Institut Bauen und Umwelt,
Berlin. ISO 14044
EN ISO 14044:2006-07, Environmental management - Life
IBU (2023) cycle assessment - Requirements and guidance (ISO
IBU (2023): P): PCR Part B: Requirements on the EPD for 14044:2006).
building hardware products. Version 2023/04, Institut Bauen
und Umwelt, Berlin. EN 1527
EN 1527:2019+A1:2021, Building hardware - Hardware for
Standards and legal documents sliding doors and folding doors - Requirements and test
methods.
EN 15804
EN 15804:2012+A2:2019+AC:2021, Sustainability of ISO 15686
construction works - Environmental product declarations - Core ISO 15686:1,-2, -7 and -8. Service life planning (various parts).
8 Environmental Product Declaration - ARGE – The European Federation of Locks and Building Hardware Manufacturers - Glass door hardware
Council Directive 75/442/EEC on waste and Council Decision
ECHA candidate list 94/904/EC establishing a list of hazardous waste pursuant to
Candidate List of substances of very high concern for Article 1(4) of Council Directive 91/689/EEC on hazardous
Authorisation, published in accordance with Article 59(10) of the waste (notified under document number C(2000) 1147).
REACH Regulation. European Chemicals Agency, Brussels.
Additional references
Ordinance on Biocide Products No. 528/2012
REGULATION (EU) No 528/2012 OF THE EUROPEAN BBSR 2017
PARLIAMENT AND OF THE COUNCIL of 22 May 2012 BBSR (2017): Nutzungsdauer von Bauteilen in
concerning the making available on the market and use of Lebenszyklusanalysen nach Bewertungssystem Nachhaltiges
biocidal products. Bauen (BNB). Version vom 24.10.2017, Bundesinstitut für Bau-,
Stadt- und Raumforschung, Berlin.
European List of Waste
Commission Decision of 3 May 2000 replacing Decision ecoinvent v3.8
94/3/EC establishing a list of wastes pursuant to Article 1(a) of http://www.ecoinvent.org
9 Environmental Product Declaration - ARGE – The European Federation of Locks and Building Hardware Manufacturers - Glass door hardware
Publisher
Institut Bauen und Umwelt e.V. +49 (0)30 3087748- 0
Hegelplatz 1 info@ibu-epd.com
10117 Berlin www.ibu-epd.com
Germany
Programme holder
Institut Bauen und Umwelt e.V. +49 (0)30 3087748- 0
Hegelplatz 1 info@ibu-epd.com
10117 Berlin www.ibu-epd.com
Germany
Author of the Life Cycle Assessment
Dr. Frank Werner - Umwelt & Entwicklung + 41 (0)44 241 39 06
Kammelenbergstrasse 30 frank@frankwerner.ch
9011 St. Gallen http://www.frankwerner.ch/
Switzerland
Owner of the Declaration
ARGE – The European Federation of Locks and +49 (0)2051 9506 15
Building Hardware Manufacturers mail@arge.org
Offerstraße 12 www.arge.org
42551 Velbert
Germany
10 Environmental Product Declaration - ARGE – The European Federation of Locks and Building Hardware Manufacturers - Glass door hardware
