ENVIRONMENTAL PRODUCT DECLARATION
as per ISO 14025 and EN 15804+A2
Owner of the Declaration European Federation of Concrete Admixtures Associations a.i.s.b.l. (EFCA)
Publisher Institut Bauen und Umwelt e.V. (IBU)
Programme holder Institut Bauen und Umwelt e.V. (IBU)
Declaration number EPD-EFC-20210198-IBG2-EN
Issue date 14.08.2023
Valid to 15.12.2026
Concrete admixtures – Plasticisers and Superplasticisers
EFCA
www.ibu-epd.com | https://epd-online.com
1. General Information
EFCA Concrete admixtures – Plasticisers and
Superplasticisers
Programme holder Owner of the declaration
IBU – Institut Bauen und Umwelt e.V. European Federation of Concrete Admixtures Associations a.i.s.b.l.
Hegelplatz 1 (EFCA)
10117 Berlin Rue d'Arlon 55
Germany 1040 Brussels
Belgium
Declaration number Declared product / declared unit
EPD-EFC-20210198-IBG2-EN 1 kg of plasticizers and superplasticizers, density: 1 - 1.6 kg/l
This declaration is based on the product category rules: Scope:
Concrete admixtures, 01.08.2021 This verified EPD entitles EFCA to bear the symbol of the Institut Bauen
(PCR checked and approved by the SVR) und Umwelt e.V. It exclusively applies for the product groups referred to for
plants operated in Belgium, Finland, France, Germany, Italy, Netherlands,
Norway, Poland, Spain, Sweden, Switzerland, Turkey and the United
Issue date Kingdom by companies that are members of EFCA National Associations
in these countries and for a period of five years from the date of issue. It
14.08.2023
involves a Model EPD where the product displaying the highest
environmental impact in a group was selected for calculating the Life Cycle
Assessment. Please refer to the EFCA website www.efca.info for a list of
Valid to
National Associations.
15.12.2026
The application of this EPD is only possible for member companies of
EFCA's member associations and only for specific formulations with a total
score below the declared maximum score for a product group according to
the associated guidance document.
The owner of the declaration shall be liable for the underlying information
and evidence; the IBU shall not be liable with respect to manufacturer
information, life cycle assessment data and evidences.
The EPD was created according to the specifications of EN 15804+A2. In
the following, the standard will be simplified as EN 15804.
Verification
Dipl.-Ing. Hans Peters
(Chairman of Institut Bauen und Umwelt e.V.) The standard EN 15804 serves as the core PCR
Independent verification of the declaration and data according to ISO
14025:2011
internally X externally
Florian Pronold Matthias Schulz,
(Managing Director Institut Bauen und Umwelt e.V.) (Independent verifier)
1 Environmental Product Declaration - EFCA - Concrete admixtures – Plasticisers and Superplasticisers
2. Product
Name Value Unit
2.1 Product description/Product definition
Density /ISO 758/ 1 - 1.6 g/ml
Admixtures are liquid or powdery agents that are introduced in
Solids content /EN 480-8/ -¹ M.-%
small amounts (< 5% by mass of the cement content) to
concrete while it is being mixed and that enhance the -log 10(a H
pH value /ISO 4316/ -¹
properties of the fresh and/or hardened concrete. )
+
Plasticizers and superplasticizers are admixtures which reduce
Maximum value to be
the water content of mixed concrete without detriment to its Chloride content /EN 480-
declared by the M.-%
consistency or enhance its slump with or without change to the 10/
manufacturer
water content or cause both effects simultaneously. They can
Maximum value to be
also display a retarding effect when used as combination
Alkali content /EN 480-12/ declared by the M.-%
products.
manufacturer
The results of the Life Cycle Assessment provided in this
declaration have been selected from the product with the Corrosion behavior /EN -² μ A/cm2
highest environmental impact (worst-case scenario). The 934-1/, /EN 480-14/
product needs a declaration of performance taking into SiO2 content /EN 192-2/ -³ M.-%
consideration EN 934-2:2009+A1:2012, Admixtures for Test mix ≤ 2% by
concrete, mortar and grout – Part 2: volume above control
Air content of fresh
Concrete admixtures – Definitions, requirements, conformity, mix unless stated Vol.-%
concrete /EN 12350-7/
marking and labelling and the CE-marking. otherwise by the
For the application and use the respective national provisions manufacturer
apply.
Compressive strength /EN
-⁵ N/mm2
12390-3/
2.2 Application
Test mix ≥ 5% com-
Concrete admixtures are used as constituent materials for the
Water reduction /EN pared to control mix
production of concrete, mortar and grout (unreinforced
12350-2/, /EN 12350-5/ Superplasticizer: Test mm
concrete, reinforced and prestressed concrete, site-mixed and
Plasticizer mix ≥ 12% com-pared to
ready-mixed concrete, precast concrete).
control mix
Their application should be in line with the manufacturer's
technical documents and Declaration of Performance. Increasing / maintaining of
consistence /EN 12350-2/,
-⁶ mm
2.3 Technical Data /EN 12350-5/
Plasticizers and superplasticizers must comply with the general Superplasticizer
requirements of EN 934-1:2008 and the additional Setting time /EN 480-2/
requirements of EN 934-2:2009+A1:2012. Accelerator/Retarder -⁴ min
The corresponding requirements in line with EN 934-1:2008
Air void Characteristics in
and EN 934-2:2009+A1:2012 must be maintained.
hardened concrete /EN -⁴ mm
Constructional data 480-11/ Air entrainer
Capillary water absorption
-⁴ g/mm2
/EN 480-5/ Densifier
¹ Value will be made available to user on request
² No corrosion behaviour test is required for admixtures which
only contain active substances in the list of approved
substances to EN 934-1, Annexe A.1 and in the list of declared
substances to EN 934-1, Annexe A.2.
³ Maximum value must only be indicated when SiO2
percentage by mass > 5 %
⁴ Details not relevant for this type of admixture
⁵ Concrete plasticizer:
At 7 and 28 days: Test mix ≥ 110 % of control mix
Superplasticizer (tested at equal consistency):
At 1 day:
Test mix ≥ 140 % of control mix
At 28 days:
Test mix ≥ 115 % of control mix
Superplasticizer (tested at equal w/c ratio): At 28 days:
Test mix ≥ 90 % of control mix
⁶ Increase in consistence
Increase in slump ≥ 120 mm from initial (30 ± 10) mm
or
Increase in flow ≥ 160 mm from initial (350 ± 20) mm
Retention of consistence 30 min after the addition:
the consistency of test mix ≥ initial consistency of the control
mix
2 Environmental Product Declaration - EFCA - Concrete admixtures – Plasticisers and Superplasticisers
Performance data of the product in accordance with the
declaration of performance with respect to its essential If this product contains other carcinogenic, mutagenic,
characteristics according to EN 934-2:2009+A1:2012, reprotoxic (CMR) substances in categories 1A or 1B which are
Admixtures for concrete, mortar and grout – Part 2: Concrete not on the candidate list, exceeding 0.1 percentage by mass,
admixtures – Definitions, requirements, conformity, marking and the relevant information can be found in the safety data sheet
labelling. of the relevant product covered by this model EPD.
If the construction product (concrete admixture - Plasticizers
2.4 Delivery status and Superplasticizers) contains CMR substances in categories
Plasticizers and superplasticizers are usually supplied in liquid, 1A or 1B exceeding 0.1 percentage by mass, the respective
paste or powder form in containers made of steel or plastic. CMR substances, information on the concentration and/or
Typical container sizes are canisters containing approx. 25 kg, concentration range together with information on their
drums with approx. 200 kg or Intermediate Bulk Containers hazardous properties are listed in the safety data sheet of the
(IBC) with 1000 kg. The containers are shipped on wooden respective product.
pallets.
For larger applications, loose deliveries in tank trucks with a 3. Biocide products added to the construction product
capacity in excess of 1 tonne are also used.
Biocide products were added to this construction product, or it
2.5 Base materials/Ancillary materials
has been treated with biocide products (this then concerns a
Plasticizers and superplasticizers essentially contain either treated product as defined by the (EU) Ordinance on Biocide
lignosulphonate, naphthalene sulphonate, melamine Products No. 528/2012)
sulphonate and polycarboxylate/polycarboxylic or mixtures Usually the construction product (concrete admixture -
thereof. Defoaming agents and preservatives are added as Plasticizers and Superplasticizers) contain small amounts
minor components and auxiliaries. (< 0.5% by mass) of biocides of the product type 'in-can
Active substance concentration lies between 10 and 40% by preservatives'.
mass. The typical dosage of plasticizers lies between 0.2 and The information which active substances are contained in the
1.6% (referred to the finished product) by mass in relation to the product can be found in the safety data sheet of the relevant
cement weight. The typical dosage of superplasticizers lies product covered by this model EPD.
between 0.4 and 2.0% by mass in relation to the cement If the construction product (concrete admixture - Plasticizers
weight. and Superplasticizers) contains biocide products, the active
The products covered by this EPD typically contain the substances, information on the concentration and/or
following proportions by mass of constituent materials and concentration range, the product type together with information
auxiliaries referred to: on their hazardous properties are listed in the safety data sheet
Lignosulphonate*: max. 40 % of the respective product.
Naphthalene sulphonate*: max. 40 %
Melamine sulphonate*: max. 45 % 2.6 Manufacture
Polycarboxylate*: max. 45 % Concrete admixtures are usually manufactured by mixing
Polyarylether max. 35 % ingredients (together) in batch mode and filling containers for
Na-gluconate max. 35 % dispatch. The process follows quality standards outlined in EN
Additives: max. 5 % 934-6:2019.
Water: approx. 55 - 75 %
*Solid content 2.7 Environment and health during manufacturing
These volumes are average values and the composition of As a general rule, no environmental or health protection
products complying with the EPD can deviate from these measures other than those specified by law are necessary.
concentration levels in individual cases.
Note: For companies to declare their products within the scope 2.8 Product processing/Installation
of this EPD it is not sufficient to simply comply with the product During concrete manufacture, concrete admixtures are usually
composition shown above. The application of this EPD is only added along with the mixing water or included in premixed
possible for member companies of EFCA's member concrete.
associations and only for specific formulations with a total score Health and safety measures (eye protection, hand protection,
below the declared maximum score for a product group possibly respiratory equipment and body protection) are to be
according to the associated guidance document. taken and consistently adhered to in accordance with the
Concrete admixtures – Plasticizers and Superplasticizers are information on the safety data sheet and conditions on site.
mixtures under the chemical legislation (REACH and
2.9 Packaging
Classification, Labelling and Packaging CLP).
Reusable containers are, where practicable taken back by the
1. substances from the 'Candidate List of Substances of manufacturer and redirected into the production circuit. Empty
Very High Concern for Authorisation' (SVHC) plastic or steel containers which can no longer be used are
recyclable.
If this product contains substances listed in the candidate list Wooden reusable pallets are, where practicable taken back by
(latest version) exceeding 0.1 percentage by mass, the relevant the manufacturer or building material trader who returns them
information can be found in the safety data sheet of the to the building product manufacturer redirecting them into the
relevant product covered by this model EPD production process.
If the construction product (concrete admixture Plasticizers and
2.10 Condition of use
Superplasticizers) contains SVHC exceeding 0.1 percentage by
During the use phase, concrete admixtures are firmly bound
mass, the respective SVHC, its CAS number, information on
into the cement matrix in hardened concrete.
the concentration and / or concentration range together with
Concrete admixtures make an essential contribution towards
information on their hazardous properties are listed in the
optimizing the physical and chemical properties of concrete
safety data sheet of the respective product.
enhancing its performance, durability, economic value and
sustainability.
2. CMR substances in categories 1A and 1B
3 Environmental Product Declaration - EFCA - Concrete admixtures – Plasticisers and Superplasticisers
2.11 Environment and health during use 2.14 Re-use phase
During the use phase, concrete admixtures are firmly bound Not relevant as this declaration relates to a preliminary product.
into the cement matrix in hardened concrete.
No relevant risks are known for water, air and soil if the 2.15 Disposal
products are used as designated. Empty, dried containers are directed to the recycling process
where practicable.
2.12 Reference service life Packaging residue must be directed to proper waste disposal
Not relevant as this declaration relates to a preliminary product. taking local guidelines into consideration.
Description of the influences on the ageing of the product when Admixture residues, during the installation phase into the
applied in accordance with the rules of technology. building, are directed to landfill. Admixture applied into the
building and dismantled at the end of the product service life
cannot be separated anymore from concrete. For this reason,
2.13 Extraordinary effects
this admixture is sent directly to landfill along with concrete.
Fire The European Waste Code (EWC) applicable for the declared
Not relevant as this declaration relates to a preliminary product. product can be assimilated to the concrete EWC 170101.
Fire protection 2.16 Further information
Not relevant as this declaration relates to a preliminary product. More information is available in the manufacturers' product or
safety data sheets on the manufacturers' Web sites or on
Water request.
Not relevant as this declaration relates to a preliminary product. An electronic version of this declaration is available at
www.efca.info and www.ibu-epd.com
Mechanical destruction
Not relevant as this declaration relates to a preliminary product.
3. LCA: Calculation rules
their life cycle.
3.1 Declared Unit Module D accounts for benefits that are beyond the defined
This EPD refers to the declared unit of 1 kg concrete admixture system boundaries. Credits are generated during the
with a density of 1-1.6 kg/l in accordance with the IBU PCR 11- incineration of wastes in module A5, which are declared in
2017 Part B for concrete admixtures. module D.
The maximum dosage of Plasticizers and Superplasticizers is
2% by mass related to the cement content in the concrete. 3.3 Estimates and assumptions
The results of the Life Cycle Assessment provided in this For this EPD formulation and production data defined by EFCA
declaration have been selected from the product with the were considered. Production waste was assumed to be
highest environmental impact (worst-case scenario). disposed of to landfill without credits as a worst case.
Depending on the application, a corresponding conversion An average of plastic containers and wooden pallets was
factor such as the density to convert volumetric use to mass considered in the LCA.
must be taken into consideration.
The Declaration type is according to EN 15804: Cradle to gate 3.4 Cut-off criteria
with options, modules C1–C4, and module D. All raw materials submitted for the formulations and production
data were taken into consideration.
Declared unit
The manufacture of machinery, plant and other infrastructure
Name Value Unit required for production of the products under review was not
Declared unit 1 kg taken into consideration in the LCA.
Gross density 1000 - 1600 kg/m3 Transport of packaging materials is excluded.
Conversion factor to 1 kg - - 3.5 Background data
Data from the GaBi database 10 (SP 40 (2020) data base was
used as background data.
3.2 System boundary
Modules A1, A2 and A3 are taken into consideration in the LCA: 3.6 Data quality
- A1 Production of preliminary products Representative products were applied for this EPD and the
- A2 Transport to the plant product in the group displaying the highest environmental
- A3 Production incl. provision of energy, production of impact was selected for calculating the LCA results. The
packaging as well as auxiliaries and consumables and waste background data sets used are no more than 4 years old.
treatment Production data and packaging are based on details provided
-A5 Installation, admixtures applied into the building during A5 by the manufacturer. The formulation used for evaluation refers
phase operations and packaging disposal. to a specific product.
-C1-C2-C4-D The data quality of the background data is considered to be
The building deconstruction (demolition process) takes place in good.
C1 module which considers energy production and
3.7 Period under review
consumption in terms of diesel and all the emissions connected
with the fuel-burning process. After the demolition, admixture is Representative formulations are valid for 2019 under
transported to the end-of-life processing (C2 module) where all consideration of data from 2011.
the impacts related to the transport processes are considered.
3.8 Geographic Representativeness
For precautionary principle and as worst-case scenario,
Land or region, in which the declared product system is
disposal is the only end of life scenario considered. This is
manufactured, used or handled at the end of the product´s
modelled by landfill process (module C4) where admixtures end
4 Environmental Product Declaration - EFCA - Concrete admixtures – Plasticisers and Superplasticisers
lifespan: Europe
3.10 Comparability
Basically, a comparison or an evaluation of EPD data is only
3.9 Allocation possible if all the data sets to be compared were created
Mass allocation have been applied when primary data have according to EN 15804 and the building context, respectively
been used and implemented into the LCA model the product-specific characteristics of performance, are taken
into account. The GaBi database SP40 (2020) has been used.
4. LCA: Scenarios and additional technical information
Material loss regards the amount of admixture not used during
Characteristic product properties of biogenic carbon the application phase into the building. This amount is 1 % of
The packaging material contains biogenic carbon content which the admixture which is considered to come into module A5
has been presented below. phase. This admixture percentage is considered as waste to
Information on describing the biogenic Carbon Content at disposal and related impacts have been considered into the
factory gate LCA model and allocated to A5.
Name Value Unit
kg
Biogenic carbon content in product - End of life (C1-C4)
C
Biogenic carbon content in accompanying kg Name Value Unit
0.0032
packaging C Collected as mixed construction waste 1 kg
Landfilling 1 kg
Modules A1-A3, A5, C1, C2, C4 and D are declared.
Assembly (A5)
Name Value Unit
Other resources for packaging 0.0311 kg
Material loss 0.01 kg
5 Environmental Product Declaration - EFCA - Concrete admixtures – Plasticisers and Superplasticisers
5. LCA: Results
Disclaimer:
EP-freshwater: This indicator has been calculated as 'kg P eq' as required in the characterization model (EUTREND model, Struijs et
al., 2009b, as implemented in ReCiPe; http://eplca.jrc.ec.europa.eu/LCDN/developerEF.xhtml)
DESCRIPTION OF THE SYSTEM BOUNDARY (X = INCLUDED IN LCA; ND = MODULE OR INDICATOR NOT DECLARED; MNR =
MODULE NOT RELEVANT)
Benefits and
Construction loads beyond
Product stage Use stage End-of-life stage
process stage the system
boundaries
la ire ta m w a Ry lp p u s tro p s n a rT g n iru tc a fu n a M e h t m o rf tro p s n a rTe tis e h t o t e ta g y lb m e s s A e s U e c n a n e tn ia M ria p e R tn e m e c a lp e R tn e m h s ib ru fe R y g re n e la n o ita re p Oe s u re ta w la n o ita re p Oe s u n o itc u rts n o c -e Dn o itilo m e d tro p s n a rT g n is s e c o rp e ts a W la s o p s iD -e s u e R-y re v o c e R-g n ilc y c e Rla itn e to p
A1 A2 A3 A4 A5 B1 B2 B3 B4 B5 B6 B7 C1 C2 C3 C4 D
X X X MND X MND MND MNR MNR MNR MND MND X X MND X X
RESULTS OF THE LCA - ENVIRONMENTAL IMPACT according to EN 15804+A2: 1 kg plasticisers and superplasticisers
Parameter Unit A1-A3 A5 C1 C2 C4 D
Global Warming Potential total (GWP-total) kg CO 2 eq 1.34E+00 1.11E-01 2.79E-04 1.24E-02 1.53E-02 -4.4E-02
Global Warming Potential fossil fuels (GWP-fossil) kg CO 2 eq 1.27E+00 8.95E-02 2.66E-04 1.18E-02 1.52E-02 -4.39E-02
Global Warming Potential biogenic (GWP-biogenic) kg CO 2 eq 6.77E-02 2.18E-02 1.24E-05 5.42E-04 4.8E-05 -1.03E-04
Global Warming Potential luluc (GWP-luluc) kg CO 2 eq 9.56E-04 5.52E-06 6.39E-09 2.79E-07 4.37E-05 -3.06E-05
Depletion potential of the stratospheric ozone layer (ODP) kg CFC11 eq 4.42E-15 6.83E-17 2.84E-20 1.24E-18 5.62E-17 -4.57E-16
Acidification potential of land and water (AP) mol H+ eq 5.75E-03 3.48E-05 3.6E-06 3.73E-05 1.09E-04 -6.13E-05
Eutrophication potential aquatic freshwater (EP-freshwater) kg P eq 1.94E-06 2.61E-08 5.75E-11 2.51E-09 2.61E-08 -5.64E-08
Eutrophication potential aquatic marine (EP-marine) kg N eq 1.2E-03 2.35E-05 1.63E-06 1.72E-05 2.8E-05 -1.59E-05
Eutrophication potential terrestrial (EP-terrestrial) mol N eq 1.58E-02 1.28E-04 1.79E-05 1.89E-04 3.08E-04 -1.7E-04
Formation potential of tropospheric ozone photochemical oxidants kg NMVOC
4.61E-03 2.81E-05 4.91E-06 3.39E-05 8.48E-05 -4.56E-05
(POCP) eq
Abiotic depletion potential for non fossil resources (ADPE) kg Sb eq 8.51E-08 1.69E-09 8.06E-12 3.52E-10 1.36E-09 -7.19E-09
Abiotic depletion potential for fossil resources (ADPF) MJ 2.85E+01 3.03E-01 3.81E-03 1.66E-01 1.99E-01 -7.44E-01
m3 world eq
Water use (WDP) 1.36E-01 1.14E-02 5.27E-07 2.3E-05 1.59E-03 -4.54E-03
deprived
RESULTS OF THE LCA - INDICATORS TO DESCRIBE RESOURCE USE according to EN 15804+A2: 1 kg plasticisers and
superplasticisers
Parameter Unit A1-A3 A5 C1 C2 C4 D
Renewable primary energy as energy carrier (PERE) MJ 1.59E+00 1.42E-01 1.2E-05 5.25E-04 2.61E-02 -1.62E-01
Renewable primary energy resources as material utilization
MJ 1.17E-01 -1.17E-01 0 0 0 0
(PERM)
Total use of renewable primary energy resources (PERT) MJ 1.7E+00 2.52E-02 1.2E-05 5.25E-04 2.61E-02 -1.62E-01
Non renewable primary energy as energy carrier (PENRE) MJ 2.27E+01 1.26E+00 3.81E-03 1.67E-01 1.99E-01 -7.44E-01
Non renewable primary energy as material utilization (PENRM) MJ 5.78E+00 -9.57E-01 0 0 0 0
Total use of non renewable primary energy resources (PENRT) MJ 2.85E+01 3.03E-01 3.81E-03 1.67E-01 1.99E-01 -7.44E-01
Use of secondary material (SM) kg 0 0 0 0 0 0
Use of renewable secondary fuels (RSF) MJ 0 0 0 0 0 0
Use of non renewable secondary fuels (NRSF) MJ 0 0 0 0 0 0
Use of net fresh water (FW) m3 4.2E-03 2.84E-04 2.16E-08 9.41E-07 5.02E-05 -1.88E-04
RESULTS OF THE LCA – WASTE CATEGORIES AND OUTPUT FLOWS according to EN 15804+A2:
1 kg plasticisers and superplasticisers
Parameter Unit A1-A3 A5 C1 C2 C4 D
Hazardous waste disposed (HWD) kg 3.55E-08 1.61E-10 3.7E-13 1.62E-11 3.03E-09 -2.97E-10
Non hazardous waste disposed (NHWD) kg 4.73E-02 2.04E-03 3.9E-07 1.7E-05 1E+00 -3.43E-04
Radioactive waste disposed (RWD) kg 5.07E-04 7.91E-06 4.09E-09 1.79E-07 2.27E-06 -5.54E-05
Components for re-use (CRU) kg 0 0 0 0 0 0
Materials for recycling (MFR) kg 0 0 0 0 0 0
Materials for energy recovery (MER) kg 0 0 0 0 0 0
Exported electrical energy (EEE) MJ 0 1.85E-01 0 0 0 0
Exported thermal energy (EET) MJ 0 3.36E-01 0 0 0 0
RESULTS OF THE LCA – additional impact categories according to EN 15804+A2-optional:
1 kg plasticisers and superplasticisers
Parameter Unit A1-A3 A5 C1 C2 C4 D
Incidence of disease due to PM emissions (PM) Disease ND ND ND ND ND ND
6 Environmental Product Declaration - EFCA - Concrete admixtures – Plasticisers and Superplasticisers
incidence
Human exposure efficiency relative to U235 (IR) kBq U235 eq ND ND ND ND ND ND
Comparative toxic unit for ecosystems (ETP-fw) CTUe ND ND ND ND ND ND
Comparative toxic unit for humans (carcinogenic) (HTP-c) CTUh ND ND ND ND ND ND
Comparative toxic unit for humans (noncarcinogenic) (HTP-nc) CTUh ND ND ND ND ND ND
Soil quality index (SQP) SQP ND ND ND ND ND ND
Potential Human exposure efficiency relative to U235, Disclaimer 1 – This impact category deals mainly with the eventual impact of low
dose ionizing radiation on human health of the nuclear fuel cycle. It does not consider effects due to possible nuclear accidents,
occupational exposure nor radioactive waste disposal in underground facilities. Potential ionizing radiation from the soil, from radon
and (from some construction materials is also not measured by this indicator.
ADP minerals & metals, ADP fossil, WDP, ETF-fw, HTP-c, HTP-nc, SQP, Disclaimer 2 – The results of this environmental impact
indicator shall be used with care as the uncertainties on these results are high or as there is limited experience with the indicator.
Additional environmental impact indicators (suggested by EN15804+A2, table 4) are not declared in the EPD.
The results of this environmental impact indicator shall be used with care as the uncertainties on these results are high and as there is
limited experience with the indicator (see ILCD classification in EN 15804, table 5). For this reason, results based on these indicators
are not considered suitable for decision-making process and are thus not declared in the EPD.
6. LCA: Interpretation
When considering upstream production and transport of pre- (HDPE) is the main contributor for all indicators followed by
products as well as manufacturing of the concrete admixture incineration of wood packaging. This module accounts also for
(modules A1-A3), the main driver of impacts in all categories is the calorific value of the packaging considered as an output
the production of pre-products (module A1), generally more and therefore with a negative value. This influence PENRM,
than 75 %. non-renewable energy content by plastic packaging and PERM,
For global warming potential (GWP) about 80 % the impacts renewable energy content by wood packaging.
are from pre-products production processes and related Considering the entire end of life modules, landfill for
chemical precursors. The manufacturing process is the second construction wastes is the main contributor for all the impact
contributor (less than 8 % of the total GWP). Important considered, followed by the truck used for transporting the
contributors to this indicator during the manufacturing process waste from the building site to the landfill.
are European electricity mix production consumed during the C1 module: the combustion of fuel occurring during demolition
admixture production process (module A3) and the plastic processes is the main contributor for this module and for all the
produced and consumed for final product packaging. European impacts considered.
electricity grid mix is an important contributor to ozone depletion C2 module:
potential (31 %) and even for eutrophication freshwater (6%). trucks used for waste transport and related combustion
Renewable primary energy demand (PERT) is influenced by emissions are the main contributor for all impacts considered.
electricity production (about 28%) and for the rest by pre- C4 module:
products production. Non-renewable primary energy demand landfill process and in particular energy consumed for landfill
(PENRT) is influenced almost only by pre-products production management and operation is the main contributor for all the
(about 91%) and electricity for 4 %. Treatment of production impacts considered.
waste has negligible contribution to impacts in all categories D module is influenced by the potential credits generated
except eutrophication freshwater (20 %), where landfilling of during installation module (A5), thanks to the energy produced
production waste has an influence. Packaging production has by the incineration processes used for packaging disposal and
an influence mainly only for resource use, mineral and metals secondly by the incineration of the admixture residue when this
(7%). material can be incinerated (thanks to its calorific value). If the
The other life cycle phases have minor influence, generally admixture has a calorific value, it can be sent to incineration
lower than 8 %. because during this phase, the residual admixture is not melted
A5 module is mainly dominated by the incineration process of with concrete.
packaging wastes, in particular the incineration of plastic
7. Requisite evidence
As this involves a declaration of preliminary products, special Documented verification
tests and evidence within the framework of drawing up this Documented verification differs depending on the application.
Model Environmental
Product Declaration have not been carried out or provided. 7.1
8. References
Candidate list CPR
Candidate list List of those eligible for approval substances of Construction Production Regulation (EU) No 305/2011 of the
very high concern to the European Chemicals Agency, as of European Parliament and of the council of 9 March 2011 laying
July 2021. down harmonised conditions for the marketing of construction
products and repealing Council Directive 89/106/EEC
CLP
Regulation (EC) No 1272/2008 of the European Parliament and EN ISO 9001:2015
of the Council on classification, labelling and packaging of EN ISO 9001:2015, Quality management systems –
substances and mixtures, as of Febrary 03-2021 Requirements (ISO 9001:2015)
7 Environmental Product Declaration - EFCA - Concrete admixtures – Plasticisers and Superplasticisers
EN 196-2:2013 EN 934-6:2019, Admixtures for concrete, mortar and grout –
EN 196-2:2013, Test methods for cement – Part 2: Chemical Part 6: Sampling, assessment and verification of the constancy
analysis of cement of performance
EN 206:2013+A1:2016 EN 12350-2:2019
EN 206:2013+A1:2016, Concrete – Part 1: Specification, EN 12350-2:2019, Testing fresh concrete – Part 2: Slump test
performance, production and conformity
EN 12350-5:2019
EN 480-1:2014 EN 12350-5:2019, Testing fresh concrete – Part 5: Flow table
EN 480-1:2014, Admixtures for concrete, mortar and grout – test
Test methods – Part 1: Reference concrete and reference
mortar for testing EN 12350-7:2019
EN 12350-7:2019, Testing fresh concrete – Part 7: Air content –
EN 480-2:2006 Pressure methods
EN 480-2:2006, Admixtures for concrete, mortar and grout –
Test methods – Part 2: Determination of setting time EN 12390-3:2019
EN 12390-3:2019, Testing hardened concrete – Part 3:
EN 480-4:2005 Compressive strength of test specimens
EN 480-4:2005, Admixtures for concrete, mortar and grout –
Test methods – Part 4: Determination of bleeding of concrete EN 14487-1:2005
EN 14487-1:2005, Sprayed concrete – Part 1: Definitions,
EN 480-5:2005 specifications and conformity
EN 480-5:2005, Admixtures for concrete, mortar and grout –
Test methods – Part 5: Determination of capillary absorption EN 15804: 2012+A2:2019
EN 15804: 2012+A2:2019, Sustainability of construction
EN 480-6:2005 works -Environmental Product Declarations - Core rules for the
EN 480-6:2005, Admixtures for concrete, mortar and grout – product category of construction products
Test methods – Part 6: Infra red analysis
EU Biocidal Products Regulation (No. 528/2012)
EN 480-8:2012 The EU Biocidal Products Regulation (No. 528/2012) Guidance
EN 480-8:2012, Admixtures for concrete, mortar and grout – document for ASD
Test methods – Part 8: Determination of the conventional dry industries (January 2016)
material content
EWC/AVV waste code
EN 480-10:2009 Directive governing introduction of the European Waste
EN 480-10:2009, Admixtures for concrete, mortar and grout – Catalogue http://www.ngs-mbh.de/zs/eak.html
Test methods – Part 10: Determination of water-soluble chloride
content GaBi 10 software & documentation
Data base for Life Cycle Engineering LBP, University of
EN 480-11:2005 Stuttgart and Sphera, documentation of GaBi 10 data sets
EN 480-11:2005, Admixtures for concrete, mortar and grout – http://documentation.gabi-software.com/, 2020
Test methods - Part 11: Determination of air void characteristics
in hardened concrete IBU 2021
Institut Bauen und Umwelt e.V.: General Instructions for the
EN 480-12:2005 EPD programme of Institut Bauen und Umwelt e.V. EPD
EN 480-12:2005, Admixtures for concrete, mortar and grout – programme. Version 2.0. Berlin: Institut Bauen und Umwelt
Test methods – Part 12: Determination of the alkali content of e.V., 2021 www.ibu-epd.com
admixtures
ISO 758:1976
EN 480-14:2006 ISO 758:1976, Liquid chemical products for industrial purposes;
EN 480-14:2006, Admixtures for concrete, mortar and grout – Determination of density at 20 °C
Test methods – Part 14: Determination of the effect on
corrosion susceptibility of reinforcing steel by potentiostatic ISO 4316:1977
electro-chemical test ISO 4316:1977, Surface active agents; Determination of the pH
value of aqueous solutions; Potentiometric method
EN 934-1:2008
EN 934-1:2008, Admixtures for concrete, mortar and grout – PCR Part A
Part 1: Common requirements Product Category Rules for Building-Related Products and
Services, Part A: Calculation Rules for the Life Cycle
EN 934-2:2009+A1:2012 Assessment and Requirements on the Project report, Version
EN 934-2:2009+A1:2012, Admixtures for concrete, mortar and 1.1, Institut Bauen und Umwelt e.V., 2021-01
grout – Part 2: Concrete admixtures – Definitions,
requirements, conformity, marking and labelling PCR Part B
Product Category Rules for Construction Products, Part B:
EN 934-5:2007 Requirements on the EPD for concrete admixtures, 2017-11
EN 934-5:2007, Admixtures for concrete, mortar and grout –
Part 5: Admixtures for sprayed concrete – Definitions, REACH Regulation
requirements, conformity, marking and labelling Regulation (EU) No 1907/2006 of the European Parliament and
of the Council of 18 December 2006 concerning the
EN 934-6:2019 Registration, Evaluation, Authorisation and Restriction of
8 Environmental Product Declaration - EFCA - Concrete admixtures – Plasticisers and Superplasticisers
Chemicals (REACH) in the EPD do not need to be listed here again.
The literature referred to in the Environmental Product The current version of PCR Part A and PCR Part B of the PCR
Declaration must be listed in full.Standards already fully quoted document on which they are based must be referenced.
9 Environmental Product Declaration - EFCA - Concrete admixtures – Plasticisers and Superplasticisers
Publisher
Institut Bauen und Umwelt e.V. +49 (0)30 3087748- 0
Hegelplatz 1 info@ibu-epd.com
10117 Berlin www.ibu-epd.com
Germany
Programme holder
Institut Bauen und Umwelt e.V. +49 (0)30 3087748- 0
Hegelplatz 1 info@ibu-epd.com
10117 Berlin www.ibu-epd.com
Germany
Author of the Life Cycle Assessment
Sphera Solutions GmbH +49 711 341817-0
Hauptstraße 111- 113 info@sphera.com
70771 Leinfelden-Echterdingen www.sphera.com
Germany
Owner of the Declaration
European Federation of Concrete Admixtures -
Associations a.i.s.b.l. (EFCA) secretary@efca.info
Rue d'Arlon 55 www.efca.info
1040 Brussels
Belgium
10 Environmental Product Declaration - EFCA - Concrete admixtures – Plasticisers and Superplasticisers
