ENVIRONMENTAL PRODUCT DECLARATION
as per ISO 14025 and EN 15804+A2
Owner of the Declaration ONDULINE SA
Publisher Institut Bauen und Umwelt e.V. (IBU)
Programme holder Institut Bauen und Umwelt e.V. (IBU)
Declaration number EPD-OND-20230363-ICD1-EN
Issue date 22.03.2024
Valid to 21.03.2029
Corrugated bitumen sheets and tiles for roofing application
ONDULINE SA
www.ibu-epd.com | https://epd-online.com
1. General Information
ONDULINE SA Corrugated bitumen sheets and tiles for roofing
application
Programme holder Owner of the declaration
IBU – Institut Bauen und Umwelt e.V. ONDULINE SA
Hegelplatz 1 Quai Gallieni 24
10117 Berlin 92150 SURESNES
Germany France
Declaration number Declared product / declared unit
EPD-OND-20230363-ICD1-EN 1m² corrugated bitumen sheets for roofing application
This declaration is based on the product category rules: Scope:
Corrugated bitumen materials for roofing and external wall This Life Cycle Assessment study is relevant for corrugated bitumen
cladding, 01.08.2021 sheets and tiles produced in the manufacturing plants of Onduline-SA
(PCR checked and approved by the SVR) located in Brazil, Malaysia, Poland, Spain and Turkey. This EPD
represents an average EPD, where a weighted average product (with an
average grammage of 3.15 kg/m²) is formed based on data provided by
Issue date the above-mentioned plants. In this study, the data collected refer to the
years 2020 to 2022.
22.03.2024
The owner of the declaration shall be liable for the underlying information
and evidence; the IBU shall not be liable with respect to manufacturer
information, life cycle assessment data and evidences.
Valid to
21.03.2029 The EPD was created according to the specifications of EN 15804+A2. In
the following, the standard will be simplified as EN 15804.
Verification
The standard EN 15804 serves as the core PCR
Independent verification of the declaration and data according to ISO
14025:2011
internally X externally
Dipl.-Ing. Hans Peters
(Chairman of Institut Bauen und Umwelt e.V.)
Florian Pronold Dr.-Ing. Nikolay Minkov,
(Managing Director Institut Bauen und Umwelt e.V.) (Independent verifier)
1 Environmental Product Declaration - ONDULINE SA - Corrugated bitumen sheets and tiles for roofing application
2. Product
2.1 Product description/Product definition 2.3 Technical Data
The products covered by this EPD are corrugated bitumen Onduline SA's Corrugated Bitumen Sheets and Tiles are
sheets and corrugated bitumen tiles, which are made from produced and delivered according to the requirements of the
cellulose fibres and bitumen. Bitumen is used to give the standard EN 534.
products their waterproofing properties. Corrugated bitumen For further details, see Technical Data Sheets at
sheets and tiles can be produced in a variety of sizes and http://www.onduline.com.
colours. Tiles are smaller than roofing sheets. These products
Constructional data
are intended for roofing applications.
Name Value Unit
The sales-weighted average weight of finished sheets and tiles Length 970 - 2015 mm
is 3.15kg per m². Width 400 - 1070 mm
Thickness 2.1 - 3.5 mm
The list of product families covered by this EPD is detailed
Grammage 2.58 - 3.98 kg/m2
below:
MALAYSIA: Performance data of the product in accordance with the
ONDULINE CLASSIC DR and DRC / ONDULINE CLASSIC declaration of performance with respect to its essential
235 / ONDUCASA (ONDUTILE 57) / ONDULINE TILE / characteristics according to EN 534 + A1, May 2010,
ONDULINE TILE IDN / ONDULINE EASYLINE / ONDUVILLA Corrugated bitumen sheets - Product specification and test
TILES methods. ONDUVILLA tiles are under European Technical
BRAZIL: Assessment/ETA-10/0018.
ONDULINE CLASSIC SR and DR and DRC / ONDULINE MAIS
2.4 Delivery status
/ ONDULINE CLASSIC 8 / TAPUME / ONDUVILLA /
ONDULINE STILO Onduline Corrugated Bitumen Sheets are delivered on pallets
POLAND: only. They are packaged by 100 or 150 or 300 or 420 sheets
ONDULINE CLASSIC range / ONDULINE EASYFIX / per pallets. Onduline Corrugated Bitumen Tiles are packaged in
ONDULINE EASYFIX VERNIS / ONDULINE EASYFIX bundles (7, 10 or 15 pieces of tiles per bundle). Bundles are
COMPACT / ONDULINE EASYFIX COMPACT VERNIS / delivered on pallets, 81 bundles per pallet (10 tiles).
ONDULINE EASYFIX COMPACT S9 / ONDULINE
2.5 Base materials/Ancillary materials
EASYSTYLE / ONDULINE EASYLINE / ONDULINE BASE 9 /
ONDULINE BASE 9 VERNIE / ONDULINE BASE STANDARD Name Value Unit
ECO 10 / ONDULINE BASE STANDARD ECO 9 / ONDULINE Waste paper / cardboard (post-consumer
43-53 %
DURO SX 35 / ONDULINE DIY 8 / BITULINE / ONDULINE 8 / recycled material content)
ONDEVER 63 / ONDALUX ECO VERNIE Bitumen 38*-48 %
SPAIN:
Resin 1-4 %
ONDULINE CLASSIC range / ONDULINE DR 32 / ONDULINE
approx.
BASE STANDARD 9 / ONDULINE ECO 10 / G76/K11 and Others %
2.3
K11S / ONDULINE U 18 / G95 / ONDULINE CLASSIC 235 / BT
190 SPANISH EXPORT / ONDULINE U21 / ONDUVILLA *: 38 % in case of thick additional coating.
TURKEY:
ONDULINE CLASSIC HR SR and DR / ONDULINE ZIGANA The product components are waste paper/cardboard, bitumen,
and ZIGANA X-TREME/ ONDULINE BASE STANDARD ECO resin, pigment, binder, paint loads, drainage agent, antifoaming
10 / ONDULINE BASE STANDARD ECO 9 / ONDURA HR 10 / agent/defoamer, dispersing agent, biocide and pH regulator.
ONDURA HR 9 / ONDURA HALF / ONDULINE ANDROMEDA / The sales-weighted average weight of finished sheets and tiles
ONDUVILLA / ONDULINE XHR / ONDULINE FIT / ONDULINE is 3.15kg per m².
HR-B / ONDURA ZIGANA
The products covered by this EPD do not contain substances
For the placing on the market of the product in the European listed in the 'Candidate List of Substances of Very High
Union/European Free Trade Association (EU/EFTA) (with the Concern for Authorisation' (date: 14/06/2023) exceeding 0.1
exception of Switzerland) Regulation (EU) No. 305/2011 (CPR) percentage by mass. These construction products are not a
applies. The corrugated bitumen sheets need a declaration of substance or mixture under the chemical law (REACH).
performance taking into consideration NF EN 534+A1 May 1,
2010 Corrugated bitumen sheets - Product specification and The products covered by this EPD do not contain other CMR
test methods and the CE-marking. Whereas the corrugated substances in categories 1A or 1B which are not on the
bitumen tiles need a declaration of performance taking into candidate list, exceeding 0.1 percentage by mass.
consideration ETA-10/0018/ and the CE-marking.
Coating additives have been added and remain on the
2.2 Application references covered by this EPD:
Corrugated bitumen sheet and tile's main function is to provide
• Octylisothiazolinone (OIT), biocide (CAS number:
water tightness on pitched roofs and walls. They can be applied
26530-20-1),
on wooden or metallic battens and purlins but also on full
• Terbutryn, biocide (CAS number: 886-50-0),
decks. The type of substructure has to be chosen according to
• Zinc pyrithione, biocide (CAS number: 13463-41-7),
the shape of the roof. They should be laid onto the substructure
• Polyethylenimine, hydrophobic agent (CAS number:
staggered and overlapped. They can be combined with several
9002-98-6).
insulation systems.
Octylisothiazolinone (2-octyl-isothiazol-3(2H)-one) is a chemical
compound belonging to the isothiazolinone class of broad-
2 Environmental Product Declaration - ONDULINE SA - Corrugated bitumen sheets and tiles for roofing application
spectrum microbiocides. roof, which is what we call "overlapping losses". See below for
ONDULINE SA's instructions on overlapping.
Octyl refers to the octyl group, which is a functional group
consisting of 8 carbon atoms. Isothiazolinone is a type of
heterocycle containing a five-membered ring composed of three
carbon atoms, one nitrogen atom and one sulphur atom.
Terbutryn is an aromatic heteromonocyclic compound
containing a methylthio-1,3,5-triazine and a diamino-1,3,5-
triazine.
2.9 Packaging
The final products are put onto wooden pallets and then
Zinc pyrithione is a coordination complex of zinc : zinc ; 1-
shrinkwrapped with polypropylene stretch foil and necessary
oxidopyridin-1-ium-2-thiolate.
registrations are done before the products are stored in the
warehouse.
No other ancillary materials or additives remain on the
products.
Possible reuse, recycling, energy recovery, and disposal routes
2.6 Manufacture of packaging materials :
Corrugated bitumen materials as sheets and tiles are made • For polypropylene stretch foil, it is considered that ratios
mainly from a single layer of natural cellulose fibres (secondary are: 28,2% landfill, 50,4% incineration with energy
material) that are recycled from all sources of wastepaper and recovery, 21,4% recycling and 0% re-use. A generic
cardboard, pre-pigmented with resin and colouring, and distance of 50km is considered between dismantling site
impregnated with bitumen, under pressure and heat. and waste treatment sites.
• For woodden pallets, it is considered that ratios are:
The production stage contains A1 (extraction, processing, 20% landfill, 31% incineration with energy recovery, 7%
production of raw materials), A2 (Transport to the manufacturer recycling and 42% re-use. It is also considered that the
and internal transport) and A3 (Manufacturing processes) transport distance from the dismantling site to the reuse
modules. site equals 200 km, whereas the transport distance to
Manufacturing steps of corrugated bitumen sheets and tiles are every other waste treatment sites (landfill, incineration
defined in detail as follows. The production process is the same and recycling) is considered to be 50km.
for all sites. For both, the manufacturing process is composed
of two main sections: 2.10 Condition of use
During use, erosion causes 10 % of the roofing sheet weight
• Cardboard production section:
loss.
The incoming wastepaper is sorted, turned into pulp and
drained. All along, processes of degassing and impurity
2.11 Environment and health during use
separation are realised. Afterwards, the pulp made of
The erosion during the use phase induces the dispersion of 5
fibres of cellulose and fillers is shaped and coloured. It
% of bitumen and 5 % of cardboard by rainwater.
undergoes primary coating (application of colour, resin
and pigment-based) and corrugation processes. 2.12 Reference service life
Cardboards are then heated and completely dried by
Service life has been declared by the manufacturer in line with
natural gas. The cardboards are cut into required
the BBSR table, the PCR (Part B, 2.12) and 15804+A2. It is
dimensions and passed onto the impregnation stage.
also based on the experience of roofing sheets and tiles
manufacture and supply. The service life is set at 25 years for
• Impregnation Section:
roofing applications.
In this section, cardboard gains its waterproofing
property. It is completely saturated with bitumen at high
A service life in accordance with the BBSR table is not a
temperatures. After impregnation, the sheets undergo
reference service life (RSL) according to ISO 15686.
curing and cooling operations –corrugated bitumen tiles
are cut to dimensions.
The service life declared by the manufacturer only applies for
For the packaging process, the finished products are put
the declared service life conditions.
onto pallets and then shrink-wrapped with
Polypropylene stretch foil.
This means that the product will meet its functional
requirements for 25 years before replacement.
2.7 Environment and health during manufacturing
ONDULINE SA's plants are certified ISO 14001 : 2004 2.13 Extraordinary effects
(Environmental management systems — Requirements with
Fire
guidance for use). Moreover, ONDULINE SA's plant located in
For all corrugated bitumen sheets and tiles manufactured by
Turkey is certified ISO 45001:2018 (Occupational health and
ONDULINE SA, the class of fire performance is E. External fire
safety management systems — Requirements with guidance
performance according to EN 13501-5 is Froof for every
for use.
product except ONDULINE HR B and ONDULINE ZIGANA
Xtrem that are Broof (t1).
2.8 Product processing/Installation
During assembly, finished product packaging as well as Fire protection
installation scraps are sent to waste treatment, electric Name Value
screwdrivers are used to install roofing sheets and tiles and
Building material class E
their fixings. This stage also induce overlapping losses. As a
Burning droplets d2
matter of fact, when laying Onduline corrugated bitumen
sheets, the manufacturer requires the sheets to be overlapped Smoke gas development -
to ensure that the roof is watertight. These overlaps mean that
more than 1sqm of sheet is needed to properly cover 1sqm of
3 Environmental Product Declaration - ONDULINE SA - Corrugated bitumen sheets and tiles for roofing application
customers.
Water
As already mentionned above, rainwater induces erosion of 10 2.15 Disposal
% of the roofing corrugated bitumen sheets and tiles. ONDULINE SA confirmed that a 100% landfill scenario shall be
considered. After an internal survey carried out by ONDULINE
Mechanical destruction SA, it has been shown that when dismantling their roofs, clients
In the event of an accidental fire, fumes are released (soot, CO, would send their corrugated bitumen sheets and tiles directly to
CO2, etc.). the waste collection site to be buried. Corrugated bitumen
sheets & tiles are classified: 17 03 02 (bituminous mixtures).
2.14 Re-use phase
Reuse, recycling and incineration with energy recovery are 2.16 Further information
possible practices but have not been considered because they For further information, please contact ONDULINE SA through
are not representative of the practices of ONDULINE SA's its website at http://www. onduline.com
3. LCA: Calculation rules
reference for the EPD.
3.1 Declared Unit
This EPD refers to a functional unit defined as follows: 1m² This declaration is classified as an 'average product' as
corrugated bitumen sheets for roofing application to ensure calculated from overall production in several of the
waterproofing and weather protection for a minimum slope of manufacturer's plants according to PCR Part A : Calculation
9% over 25 years. Rules for the Life Cycle Assessment and Requirements on the
Project Report according to EN 15804+A2:2019 (version 1.3),
The environmental profile is based on a weighted average, as 31 August 2021; www.bau-umwelt.de.
the LCA results refer to the specified functional unit.
3.2 System boundary
Declared unit and mass reference
The system boundary covers the entire life cycle of the product
Name Value Unit
from extraction of raw materials to the disposal of the product
Grammage (weighted average value between 3.15 kg/m2 (cradle to grave). It also includes the module D.
2020 and 2022)
Declared unit 1 m2 3.3 Estimates and assumptions
All raw materials used by ONDULINE SA have been
Layer thickness (weighted average value
0.0029 m approximated by datasets found on Ecoinvent 3.8 database.
between 2020 and 2022)
For a more detailed study, an on-site collection of data (i.e. a
collection of data on the production sites of ONDULINE SA's
This study aims to find the environmental impacts generated by suppliers) would be required to acquire detailed information on
ONDULINE SA products throughout their life cycle. For this, the the products identified as having a high level of impact.
standards ISO 14040, ISO 14044, EN 15804 have been
complied with regarding the quality of data for the following Waterproofing properties of ONDULINE SA's products depend
criteria: on bitumen type (road bitumen). The grades selected by
• Time factor – LCI data are based on: ONDULINE are such that the bitumen does not remain on the
- Where available, data collected specifically for this surface of the sheet, allowing the material to be waterproof and
study at ONDULINE SA production sites in Spain, homogenous as required by EN 534 standard. We have
Brazil, Malaysia, Poland and Turkey. These data assumed that the dataset found on Ecoinvent 3.8 database
correspond to the average production based on the matched the bitumen formulation purchased by ONDULINE SA.
study of data from the years 2020-2021-2022. Instead of taking a global dataset, we narrowed the studied
- In the absence of specific data, generic data from the area to Europe (for factories in Poland and Spain), to Rest of
Ecoinvent database 3.8 Allocation, cut-off by the World (for factories in Malaysia and Turkey) and we took
Classification (2022). This database is regularly updated the Brazil dataset for the Brazilian factory. This limits the
and is representative of current processes. possible difference between averaged bitumen formulation per
studied area and purchased bitumen formulations by each
• Geographical factor:
factory.
- Specific data come from the manufacturer's production
sites in Spain, Brazil, Malaysia, Poland and Turkey.
Whenever possible country-specific data (e.g. electricity, ...)
- Generic data from the Ecoinvent database
was applied. When such data is missing, European, rest-of-the
representing European or Rest of the World processes
world or global datasets are preferred (e.g. resins, natural gas,
have been used for manufacturing stages where
etc.)
available, otherwise global data are used.
For transports: When multiple location applied to the same raw
• Technological factor – material shaping technology data
material or reference of product, weighted average of the
are based on:
distances were used. All raw materials, their amount, their
- Technologies used by the manufacturer for the
distance between suppliers/producers and ONDULINE SA's
production processes of their products.
plants were collected from each plant. All sales figures were
- European or Global technologies depending on the
also collected from each plant, as well as the related transport
production site considered in the case of generic data.
distances. All transports by lorry as well as transports by light
The EPD covers individual products, which are grouped by type
commercial vehicle have been modelled with a calculated
of application and product families. To evaluate the impacts of
Global dataset. Transports by container ship were modelled
the group of products, each product has been evaluated
with Ecoinvent Global dataset.
individually. For all typologies, the created average product
according to the distribution of global sales is used as a
All the bitumen waste from disposal phase have been modelled
4 Environmental Product Declaration - ONDULINE SA - Corrugated bitumen sheets and tiles for roofing application
as going to sanitary landfill. Although some ONDULINE SA's data has been taken from the Ecoinvent database 'Ecoinvent
customers do not send their corrugated bitumen sheets to 3.8 – allocation cut-off by classification'.
landfill when they are dismantled, but rather to recycling or
reuse, we have conservatively assumed that all flows went to 3.6 Data quality
landfill. ONDULINE SA did not have figures to give to EVEA. For this average EPD, geographical, technical, temporal as well
as methodological representativity have been met:
3.4 Cut-off criteria
• Geographical coverage is global,
The cut-off criteria used for this study follow the guidelines set
• Production data are based on the years 2020 to 2022
out in the PCR which conform to the EN15804, as follows:
(this study is based on 3-year averaged data, as
- All inputs and outputs to a (unit) process are included in the
provided by ONDULINE SA),
calculation where the data is available.
• Technologies used by the manufacturer for the
- A maximum of 1 % of the total mass per unit process may be
production processes have been used in the calculation,
omitted.
and European or Global technologies depending on the
- A maximum of 1 % of the total renewable and non-renewable
production site have been considered when generic
energy for a unit process may be omitted.
data where to be used,
- A maximum of 5 % of the total energy usage and mass per
• Data quality assessment is compliant to EN15804+A2
module may be omitted.
standard.
All data was collected by ONDULINE SA in kg per kg of
This study does not include infrastructures, production tools,
product. The data was reported in kg per sqm in the Simapro
factory construction, lighting, heating, cleaning, administration
tool.
department or employee transport, except in the case of data
included in the generic databases.
Variability studies have shown that sales-weighted average
• Modules A1-A5 products per country can have an impact of -11% to +17%
A1 & A2: The raw and secondary materials as well as their regarding average GWP (the highest rates are for Malaysia and
transport have been included in the calculation. the lowest rates are for Spain). They have also shown that the
Packaging of waste paper (steel strapping around stacks of references alone can have an impact of -43% to +85%
waste paper) as well as its transport have been included in the regarding average GWP (highest rate is that of a Malaysian
calculation. The other raw materials packaging and their reference and lowest rates is that of a Brazilian reference).
transport were negligible and have not been included in the
calculation. Malaysia has the highest overall carbon footprint. This is mainly
A3: Energy consumption, production goods, production losses due to its electricity consumption (highest of the 5 countries
and wastes, finished product packaging and the import of studied), its energy mix, the averaged mass per square meter
fixings have been included in the calculation. of finished product (2nd highest of the 5 countries) and the
Internal transport via forklift within the factory (Forklifts transport distance of the finished product (2nd highest of the 5
employed are diesel, LPG or/and propane driven) has not been countries).
included in the calculationdue to the lack of annual fuel
consumption figures and because this consumption is 3.7 Period under review
negligible regarding the impact of raw materials. The period under review for the collection of production data
A4: Transport of the finished products, their fixings and their and the resulting averages runs from 2020 to 2022.
packaging to the stockist and then the construction site have
3.8 Geographic Representativeness
been included in the calculation.
A5: Screwdriver electric consumption during installation, Land or region, in which the declared product system is
installation scraps (cutting scraps), installation losses manufactured, used or handled at the end of the product´s
(overlapping) and finished product packaging waste have been lifespan: Global
included in the calculation.
• Module B1 3.9 Allocation
All input and output flows have been considered. The manufacturing process does not generate any
VOC emissions have been neglected, moreover no data was simultaneous co-products. No allocation has been made on the
available. production data.
• Module B2
3.10 Comparability
According to the data provided by ONDULINE SA, the
Basically, a comparison or an evaluation of EPD data is only
consumption of water used when cleaning the roofs can be
possible if all the data sets to be compared were created
omitted.
according to EN 15804 and the building context, respectively
• Modules B3-B7
the product-specific characteristics of performance, are taken
There are no input or output flows associated with these
into account. Ecoinvent database 'Ecoinvent 3.8 – allocation
modules for the products considered.
cut-off by classification' has been used.
• Modules C1-C4
All input and output flows have been considered.
• Module D
Module D has been considered for this report. It does not
include the packaging (Polypropylene stretch foil and wood
pallet).
3.5 Background data
The data used to create the model within the LCA software
Simapro 9.5 has been provided by ONDULINE SA. Generic
5 Environmental Product Declaration - ONDULINE SA - Corrugated bitumen sheets and tiles for roofing application
4. LCA: Scenarios and additional technical information
The waste treatment of finished product packaging
Characteristic product properties of biogenic carbon (polypropylene stretch foil and wood pallets) has been
In this LCA, biogenic carbon content has been quantified and modelled with generic data created by EVEA. For wooden
declared for wooden pallets (packaging) and cardboard pallets, it is considered that ratios are: 20% landfill, 31%
contained in the corrugated bitumen sheets and tiles. incineration with energy recovery, 7% recycling and 42% re-
use. For polypropylene stretch foil, it is considered that ratios
Note: 1 kg of biogenic carbon is equivalent to 44/12 kg of CO 2. are: 28,2% landfill, 50,4% incineration with energy recovery,
21,4% recycling and 0% re-use. A generic distance of 50km is
Information on describing the biogenic carbon content at
considered between dismantling site and waste treatment sites.
factory gate
Name ValueUnit
Use or application of the installed product (B1)
kg
Biogenic carbon content in product Cardboard 0.45 During the use stage, erosion causes 10 % of the roofing sheet
C
weight loss. Thus 5 % of bitumen and 5 % of cardboard are
Biogenic carbon content in accompanying kg
0.47 taken away with rainwater. Yet, rainwater added to cardboard
packaging Wooden pallet C
induce cellulose hydrolysis which creates glucose. Erosion has
been modelled with 5% petrol discharge in water and 5 %
The following is the technical scenario information used for glucose discharge in water. However, glucose is not
declared modules. characterized in the calculation method.
Transport to the building site (A4) Name Value Unit
The transport of the final products has been modelled by Erosion (mass loss) 0.37 kg
considering their precise destinations in the world. For each Petrol discharge 0.19 kg
product family, a transport distance averaged by sales volumes
Glucose discharge 0.19 kg
for each destination has been taken. The transported mass of
packaging of the finished products as well as the transported ONDULINE SA's corrugated bitumen sheets for roofing
mass of fixings needed for the installation stage are included in application have 25 years of service lifetime.
the calculation at this stage. Lorry and container ship generic Service life
models used are globally representative. A third transport The service life declared by the manufacturer (25 years) only
model has been created here to consider a generic distance of applies for the declared service life conditions.
a 100km covered by a light commercial vehicle between the
Name Value Unit
stockist and the building site. This model is also globally
Life Span (according to BBSR) 25 years
representative.
Application roofing
Name Value Unit
Declared product properties (at
Transport distance by truck 983 km EN 534:2006+A1 -
the gate) and finishes
Transport distance by container ship 1337 km
Design application parameters See ONDULINE SA
Transport distance by light commercial vehicule 100 km
(if instructed by the technical book and
manufacturer), including the instructions on reference -
Installation into the building (A5)
references to the appropriate conditions of application
Distribution packaging consists of wooden pallets (2,54E-02
practices and application codes and use
kg/m²) and polypropylene stretch foil (1,82E-03 kg/m²).
See ONDULINE SA
An assumed quality of work,
technical book and
Electric screwdrivers are used to fix sheets and tiles to the when installed in accordance
instructions on reference -
roofing. ONDULINE SA has estimated the screwdriver's electric with the manufacturer’s
conditions of application
consumption at 0,0025 kWh per kg of installed product instructions
and use
regardless of the reference. The electric consumption is
converted in kWh per m² of product before being integrated in Outdoor environment, (for
SimaPro. As ONDULINE SA products are sold all over the outdoor applications), e.g.
world, the Ecoinvent data is representative of the world. weathering, pollutants, UV and
No specific restrictions -
wind exposure, building
Name Value Unit
orientation, shading,
Electricity consumption 0.008 kWh
temperature
Installation scraps 3 %
Usage conditions, e.g.
Overlapping losses depend on the reference of sheets and frequency of use, mechanical No specific restrictions -
tiles, for sheets they are around 17-20 % and can go up to 30 exposure
% in case of small elements (ONDUVILLA tiles). They have Maintenance e.g. required
been modelled with only a demand of overproduction to offset frequency, type and quality and No specific restrictions -
the losses. No waste treatment has been modelled. The scraps replacement of components
associated with the installation, entirely in the form of offcuts,
are estimated at 3 % by ONDULINE SA. They have been End of life (C1-C4)
modelled with overproduction to offset the scraps and with a The same energy consumption as in A5 has been considered,
waste treatment. According to ONDULINE SA's information, the given that electric screwdrivers are also used to remove sheets
end-of-life scenario to be considered for installation scraps is and tiles from the roof.Corrugated bitumen sheets, tiles and
100 % landfill. All these scraps are transported by truck to the fixings are sent by truck to their waste treatment and their
landfill site, assumed to be 50km away. It is modelled with a recycling sites 50 km away.
global lorry data. 100 % of the fixings are recycled.
100 % of the corrugated bitumen sheets and tiles are landfilled.
6 Environmental Product Declaration - ONDULINE SA - Corrugated bitumen sheets and tiles for roofing application
Name ValueUnit Recycling potentials (D), relevant scenario information
The recycling of fixings is considered in module D.
Collected separately waste type (Fixings) 0.07 kg
Module D includes the credits of the recycling of fixings (100%)
Collected separately (Corrugated bitumen sheets) 3.362 kg
from C3, considering that 26% of the fixings contain recycled
Recycling (Fixings) 0.07 kg
steel.
Landfilling (Corrugated bitumen sheets) 3.362 kg
7 Environmental Product Declaration - ONDULINE SA - Corrugated bitumen sheets and tiles for roofing application
5. LCA: Results
DESCRIPTION OF THE SYSTEM BOUNDARY (X = INCLUDED IN LCA; MND = MODULE OR INDICATOR NOT DECLARED; MNR
= MODULE NOT RELEVANT)
Benefits and
Construction loads beyond
Product stage Use stage End of life stage
process stage the system
boundaries
la ire ta m w a Ry lp p u s tro p s n a rT g n iru tc a fu n a M e h t m o rf tro p s n a rTe tis e h t o t e ta g y lb m e s s A e s U e c n a n e tn ia M ria p e R tn e m e c a lp e R tn e m h s ib ru fe R y g re n e la n o ita re p Oe s u re ta w la n o ita re p Oe s u n o itc u rts n o c -e Dn o itilo m e d tro p s n a rT g n is s e c o rp e ts a W la s o p s iD -e s u e R-y re v o c e R-g n ilc y c e Rla itn e to p
A1 A2 A3 A4 A5 B1 B2 B3 B4 B5 B6 B7 C1 C2 C3 C4 D
X X X X X X X X X X X X X X X X X
RESULTS OF THE LCA - ENVIRONMENTAL IMPACT according to EN 15804+A2: 1 m² of roof covered by corrugated bitumen
sheets for minimum slopes of 9% and a lifespan of 25 years
Parameter Unit A1 A2 A3 A4 A5 B1 B2 B3 B4 B5 B6 B7 C1 C2 C3 C4 D
GWP-total kg CO 2 -1.53E 1.29E- 1.52E 1.22E 5.67E-01 1.26E- 0 0 0 0 0 0 5.65E- 2.92E- 5.51E- 3.27E -4.68E-
eq +00 01 +00 +00 02 03 02 03 +00 02
GWP-fossil kg CO 2 1.12E 1.29E- 1.42E 1.22E 8.95E-01 0 0 0 0 0 0 0 5.63E- 2.92E- 5.5E-03 4.29E- -4.69E-
eq +00 01 +00 +00 03 02 01 02
GWP- kg CO 2 -2.66E 3.82E- 9.96E- 6.38E- -3.31E- 1.26E- 0 0 0 0 0 0 1.53E- 8.67E- 8.52E- 2.84E 6.29E-05
biogenic eq +00 05 02 04 01 02 05 06 06 +00
GWP-luluc kg CO 2 8.55E- 5.42E- 4.46E- 6.95E- 3.03E-03 0 0 0 0 0 0 0 1.35E- 1.22E- 4.3E-06 4.13E- 3.37E-05
eq 03 05 03 04 05 05 05
kg CFC11 1.05E- 1.14E- 1.94E- 6.58E- 9.95E- 1.08E- -1.41E-
ODP 2.9E-08 2.6E-07 3.17E-07 0 0 0 0 0 0 0
eq 06 07 10 09 10 08 09
1.06E- 5.72E- 5.54E- 7.19E- 2.92E- 1.21E- 2.58E- 5.44E- -2.01E-
AP mol H+ eq 5.35E-03 0 0 0 0 0 0 0
02 04 03 03 05 04 05 04 04
EP- 2.26E- 1.04E- 5.49E- 1.35E- 3.01E- 2.36E- 9.59E- 6.47E- -1.75E-
kg P eq 2.19E-05 0 0 0 0 0 0 0
freshwater 05 06 05 05 07 07 08 07 07
1.36E- 1.66E- 1.33E- 2.06E- 4.89E- 3.55E- 6.43E- 4.32E- -7.43E-
EP-marine kg N eq 1.12E-03 0 0 0 0 0 0 0
03 04 03 03 06 05 06 04 06
1.69E- 1.83E- 1.06E- 2.29E- 5.48E- 3.92E- 7.85E- 1.16E- -5.24E-
EP-terrestrial mol N eq 1.17E-02 0 0 0 0 0 0 0
02 03 02 02 05 04 05 03 04
kg
5.53E- 3.53E- 7.03E- 1.48E- 2.13E- 4.57E- -2.83E-
POCP NMVOC 5.8E-03 3.8E-03 0 0 0 0 0 0 0 1.2E-04
04 03 03 05 05 04 04
eq
1.06E- 4.54E- 4.41E- 1.15E- 2.69E- 1.03E- 2.37E- 1.28E-
ADPE kg Sb eq 6.03E-06 0 0 0 0 0 0 0 -1.5E-06
05 07 06 05 08 07 08 07
1.93E 2.02E 2.51E 4.37E- 7.92E- 8.57E- -3.96E-
ADPF MJ 7.4E+01 1.8E+01 0 0 0 0 0 0 0 7.5E-02
+00 +01 +01 01 02 01 01
m3 world
7.17E- 6.38E- 3.47E- 7.61E- 9.37E- 1.45E- 4.45E- 3.65E-
WDP eq 2.64E-01 0 0 0 0 0 0 0 1.28E-02
01 03 01 02 04 03 04 02
deprived
GWP = Global warming potential; ODP = Depletion potential of the stratospheric ozone layer; AP = Acidification potential of land and water; EP =
Eutrophication potential; POCP = Formation potential of tropospheric ozone photochemical oxidants; ADPE = Abiotic depletion potential for non-fossil
resources; ADPF = Abiotic depletion potential for fossil resources; WDP = Water (user) deprivation potential)
RESULTS OF THE LCA - INDICATORS TO DESCRIBE RESOURCE USE according to EN 15804+A2: 1 m² of roof covered by
corrugated bitumen sheets for minimum slopes of 9% and a lifespan of 25 years
Parameter Unit A1 A2 A3 A4 A5 B1 B2 B3 B4 B5 B6 B7 C1 C2 C3 C4 D
7.24E- 2.35E- 2.03E 3.37E- 1.29E 9.72E- 5.36E- 3.35E- 1.71E- -5.51E-
PERE MJ 0 0 0 0 0 0 0
01 02 +00 01 +00 03 03 03 02 02
1.35E 5.54E
PERM MJ 3E+01 0 0 0 0 0 0 0 0 0 0 0 0 0 0
+00 +00
3.07E 2.35E- 3.38E 3.37E- 6.82E 9.72E- 5.36E- 3.35E- 1.71E- -5.51E-
PERT MJ 0 0 0 0 0 0 0
+01 02 +00 01 +00 03 03 03 02 02
1.23E 1.93E 1.96E 1.18E 7.47E- 4.37E- 7.92E- 8.56E- -3.96E-
PENRE MJ 1.8E+01 0 0 0 0 0 0 0
+01 +00 +01 +01 02 01 02 01 01
5.93E- 1.46E
PENRM MJ 6.8E+01 0 0 0 0 0 0 0 0 0 0 0 0 0 0
01 +01
8.02E 1.93E 2.02E 2.64E 7.47E- 4.37E- 7.92E- 8.56E- -3.96E-
PENRT MJ 1.8E+01 0 0 0 0 0 0 0
+01 +00 +01 +01 02 01 02 01 01
1.61E 2.26E- 3.53E-
SM kg 0 0 0 0 0 0 0 0 0 0 0 0 0 0
+00 02 01
RSF MJ 0 0 0 0 0 0 0 0 0 0 0 0 0 0 0 0 0
NRSF MJ 0 0 0 0 0 0 0 0 0 0 0 0 0 0 0 0 0
1.78E- 2.04E- 9.38E- 4.56E- 1.62E- 8.84E-
FW m3 2E-04 2.5E-03 0 0 0 0 0 0 0 4.4E-05 5.3E-04
02 02 03 05 05 04
8 Environmental Product Declaration - ONDULINE SA - Corrugated bitumen sheets and tiles for roofing application
PERE = Use of renewable primary energy excluding renewable primary energy resources used as raw materials; PERM = Use of renewable primary
energy resources used as raw materials; PERT = Total use of renewable primary energy resources; PENRE = Use of non-renewable primary energy
excluding non-renewable primary energy resources used as raw materials; PENRM = Use of non-renewable primary energy resources used as raw
materials; PENRT = Total use of non-renewable primary energy resources; SM = Use of secondary material; RSF = Use of renewable secondary fuels;
NRSF = Use of non-renewable secondary fuels; FW = Use of net fresh water
RESULTS OF THE LCA – WASTE CATEGORIES AND OUTPUT FLOWS according to EN 15804+A2:
1 m² of roof covered by corrugated bitumen sheets for minimum slopes of 9% and a lifespan of 25 years
Parameter Unit A1 A2 A3 A4 A5 B1 B2 B3 B4 B5 B6 B7 C1 C2 C3 C4 D
4.87E- 1.76E- 8.59E- 2.45E- 4.45E- 2.53E- 1.11E- 1.22E- -2.48E-
HWD kg 0 0 0 0 0 0 0 4E-04
02 03 02 02 02 04 03 03 02
5.73E- 1.11E- 9.68E- 9.57E- 7.05E- 3.92E- 2.54E- 4.85E- 3.38E -6.78E-
NHWD kg 0 0 0 0 0 0 0
01 01 01 01 01 03 02 03 +00 02
1.27E- 2.59E- 1.17E- 1.41E- 2.31E- 2.87E- 5.02E-
RWD kg 4.9E-04 0 0 0 0 0 0 0 4.6E-07 2.96E-07
05 05 04 04 07 06 06
4.09E-
CRU kg 0 0 0 0 0 0 0 0 0 0 0 0 0 0 0 0
02
8.32E- 7.02E-
MFR kg 0 0 0 0 0 0 0 0 0 0 0 0 0 0 0
03 02
MER kg 0 0 0 0 0 0 0 0 0 0 0 0 0 0 0 0 0
5.24E-
EEE MJ 0 0 0 0 0 0 0 0 0 0 0 0 0 0 0 0
02
1.09E-
EET MJ 0 0 0 0 0 0 0 0 0 0 0 0 0 0 0 0
01
HWD = Hazardous waste disposed; NHWD = Non-hazardous waste disposed; RWD = Radioactive waste disposed; CRU = Components for re-use;
MFR = Materials for recycling; MER = Materials for energy recovery; EEE = Exported electrical energy; EET = Exported thermal energy
RESULTS OF THE LCA – additional impact categories according to EN 15804+A2-optional:
1 m² of roof covered by corrugated bitumen sheets for minimum slopes of 9% and a lifespan of 25 years
Parameter Unit A1 A2 A3 A4 A5 B1 B2 B3 B4 B5 B6 B7 C1 C2 C3 C4 D
Disease 7.85E- 3.64E- 1.16E- 5.56E- 2.18E- 2.51E- 4.48E- 6.27E- -2.58E-
PM 1.1E-08 0 0 0 0 0 0 0
incidence 08 08 07 08 10 09 10 09 09
kBq U235 3.02E- 8.04E- 2.74E- 7.63E- 9.13E- 3.35E- 1.82E- 3.28E- 3.33E-
IR 0 0 0 0 0 0 0 7.04E-04
eq 01 03 02 02 02 04 03 04 03
2.13E 6.88E- 5.19E 6.37E 7.51E 5.69E 1.85E- 1.56E- 2.86E- 7.47E-
ETP-fw CTUe 0 0 0 0 0 0 8.65E-02
+01 01 +00 +00 +00 +00 02 01 02 01
4.71E- 4.94E- 1.25E- 2.31E- 1.66E- 1.11E- 2.83E-
HTP-c CTUh 1.8E-09 0 0 0 0 0 0 0 2.6E-12 4.68E-10
09 11 09 09 12 11 11
1.55E- 1.59E- 1.45E- 1.92E- 1.29E- 1.37E- 3.63E- 6.75E- 4.41E-
HTP-nc CTUh 0 0 0 0 0 0 6E-11 2.83E-09
08 09 08 08 08 11 10 11 10
9.35E 1.72E 9.06E 1.21E- 2.98E- -1.93E-
SQP SQP 1.3E+00 1E+01 0 0 0 0 0 0 0 5.9E-02 2E+00
+00 +01 +00 02 01 01
PM = Potential incidence of disease due to PM emissions; IR = Potential Human exposure efficiency relative to U235; ETP-fw = Potential comparative
Toxic Unit for ecosystems; HTP-c = Potential comparative Toxic Unit for humans (cancerogenic); HTP-nc = Potential comparative Toxic Unit for humans
(not cancerogenic); SQP = Potential soil quality index
Disclaimer 1 – for the indicator 'Potential Human exposure efficiency relative to U235'. This impact category deals mainly with the
eventual impact of low-dose ionizing radiation on human health of the nuclear fuel cycle. It does not consider effects due to possible
nuclear accidents, occupational exposure or radioactive waste disposal in underground facilities. Potential ionizing radiation from the
soil, radon and from some construction materials is also not measured by this indicator.
Disclaimer 2 – for the indicators 'abiotic depletion potential for non-fossil resources', 'abiotic depletion potential for fossil resources',
'water (user) deprivation potential, deprivation-weighted water consumption', 'potential comparative toxic unit for ecosystems', 'potential
comparative toxic unit for humans – cancerogenic', 'Potential comparative toxic unit for humans - not cancerogenic', 'potential soil
quality index'. The results of this environmental impact indicator shall be used with care as the uncertainties on these results are high
as there is limited experience with the indicator.
As no RSL is declared according to ISO 15686, the LCA results of the modules B1-B2 and B6-B7 refer to a period of one year.
This EPD was created using a software tool.
6. LCA: Interpretation
For all products, the stages with the greatest environmental radiation, Human toxicity (cancer and non-cancer), Total non-
impacts are: the raw materials supply stage (A1), the renewable primary energy, Net use of fresh water, Hazardous
manufacturing stage (A3), the delivery transport stage (A4), the waste disposed, Radioactive waste disposed, Interm. & low-
installation stage (A5), the end of life – disposal phase (C4). level radioactive waste, Exported energy and Total primary
energy. It is mostly always due to the supply of bitumen, for
The raw material supply is responsible for over 20% of the some indicators, it is also due to the supply of resin and for a
impact for following indicators: Climate change – fossil, Climate few indicators it is partly due to the supply of pigments.
change - land use and change, Ozone depletion, Acidification,
Eutrophication (freshwater, marine and terrestrial), The raw material supply is also responsible for over 70% of the
Photochemical ozone formation, Resource use (minerals, impact for following indicators: Renewable primary energy used
metals and fossils), Water use, Particulate matter, Ionising as RM, Total renewable primary energy, Non-renewable
9 Environmental Product Declaration - ONDULINE SA - Corrugated bitumen sheets and tiles for roofing application
primary energy used as RM and Use of secondary material. It is products per country can have an impact of -11% to +17%
always due to the supply of cardboard, except for the indicator regarding average GWP (the highest rates are for Malaysia and
'Non-renewable primary energy used as RM', for which it is due the lowest rates are for Spain). They have also shown that the
to the supply of bitumen. references alone can have an impact of -43% to +85%
regarding average GWP (highest rate is that of a Malaysian
The manufacturing stage is responsible for over 30% of the reference and lowest rates is that of a Brazilian reference).
impact for following indicators:
Considering the high results variability, the environmental
• Climate change - land use and change, Eutrophication
profile of a sub-group of products or individual products are
(freshwater), Net use of fresh water and High-level
available upon request.
radioactive waste, due to the electric consumption,
• Land use and Renewable primary energy excl. RM, due
to the supply of wood pallets,
Climate change – fossil and Non-renewable primary
energy excl. RM, due to the consumption of natural gas,
• Hazardous waste disposed, due to the supply of fixings.
The transport stage (finished product transport – A4) is
responsible for over 25% of the impact for following indicators:
Eutrophication (marine and terrestrial), Photochemical ozone
formation, Resource use (minerals and metals), Particulate
matter, Human toxicity (non-cancer), Non-renewable primary
energy excl. RM, always and overwhelmingly due to the
delivery by light commercial vehicle from stockist to worksite.
The installation stage (A5) is responsible for over 15% of the
impact for all the indicators studied in EN15804 standard
(except Climate change – biogenic and total, Use of renewable
secondary fuels, Use of non-renewable secondary fuels, Non-
hazardous waste disposed, Materials for recycling, Materials for
energy recovery, Exported energy - gas and process), mainly
due to the overproduction needed to offset the overlapping
rates and for a few indicators, it is also due also to the end of
life of the wooden pallets.
Finally, the disposal stage (C4) is responsible for over 40% of
the impact for following indicators: Climate change – total,
Climate change – biogenic, Non-hazardous waste disposed,
due to the landfilling of waste bitumen sheets.
Distribution of impacts for the sales weighted average product
(roofing application, LCA results over the full service life)
Variability studies have shown that sales-weighted average
10 Environmental Product Declaration - ONDULINE SA - Corrugated bitumen sheets and tiles for roofing application
7. Requisite evidence
External fire performance and reaction to fire of the roofing 5:2016
systems (sheets + tiles) have been tested according to EN Measuring agency: Warrington fire, WFRGENT nv
13501-1, EN 13501-5 and test method NBN CEN/TS 1187 (test Results of the measurement: Class of external fire performance
1). is Froof for every product, except ONDULINE HR B and
ONDULINE ZIGANA Xtrem that are Broof. Class of fire reaction
Test standard: CEN/TS 1187-T1 is E for every product.
Classification standard: EN 13501-1:2016 and EN 13501-
8. References
EN 534:2006+A1:2010 Type III environmental declarations — Principles and
Corrugated bitumen sheets-Product specification and test procedures.
method
ISO 14040-44
EN 13501-1:2016 DIN EN ISO 14040:2006: Environmental management - Life
BS EN 13501-1:2016, Fire classification of construction cycle assessment - Principles and framework (ISO 14040:2006)
products and building elements - Part1: Classification using and Requirements and guidelines (ISO 14044:2006)
data from reaction to fire tests
Regulation (EU) No. 305/2011 (CPR)
EN 13501-5 Harmonised conditions for the marketing of construction
NBN EN 13501-5, Fire classification of construction products products
and building elements - Part 5: Classification using data from
external fire exposure to roofs tests Database Ecoinvent
Test method NBN CEN/TS 1187 (test 1). Ecoinvent v3.8 (2022 - Ecoinvent Centre)
EN 14964:2006 IBU 2021
Rigid underlays for discontinuous roofing – type OL - Definitions Institut Bauen und Umwelt e.V.: General Instructions for the
and characteristics EPD programme of Institut Bauen und Umwelt e.V., Version
2.0, Berlin: Institut Bauen und Umwelt e.V., 2021
EN 15804 www.ibu-epd.com
EN 15804:2012+A2:2019+AC:2021, Sustainability of
construction works — Environmental Product Declarations — PCR Part A
Core rules for the product category of construction products. Institut Bauen und Umwelt e.V., Berlin (pub.): Product Category
Rules for Construction Products from the range of
ETA-10/0018 Environmental Product Declarations of Institut Bauen und
Corrugated Bitumen Tiles – Onduvilla: 2015 Umwelt (IBU). Part A: Calculation Rules for the Life Cycle As-
sessment and Requirements on the Project Report according to
ISO 9001 : 2008 EN 15804+A2:2019 (version 1.3), 31 August 2021; www.bau-
Quality management systems — Requirements umwelt.de
ISO 14001 : 2004 PCR Part B
Environmental management systems — Requirements with Institut Bauen und Umwelt e.V., Berlin (pub.): Product Category
guidance for use. Rules for Construction Products from the range of
Environmental Product Declarations of Institut Bauen und
ISO 45001:2018 Umwelt (IBU), Part B: Requirements on the EPD for corrugated
Occupational health and safety management systems — bitumen materials for roofing and external wall cladding, 1 June
Requirements with guidance for use. 2021, www.bau-umwelt.de
ISO 14025 Software Simapro
EN ISO 14025:2011, Environmental labels and declarations — SimaPro 9.5 (2023 - Pré consultant)
11 Environmental Product Declaration - ONDULINE SA - Corrugated bitumen sheets and tiles for roofing application
Publisher
Institut Bauen und Umwelt e.V. +49 (0)30 3087748- 0
Hegelplatz 1 info@ibu-epd.com
10117 Berlin www.ibu-epd.com
Germany
Programme holder
Institut Bauen und Umwelt e.V. +49 (0)30 3087748- 0
Hegelplatz 1 info@ibu-epd.com
10117 Berlin www.ibu-epd.com
Germany
Author of the Life Cycle Assessment
EVEA +33 2 28 07 87 00
rue Arthur III, 11 evea@evea-conseil.com
44200 Nantes www.evea-conseil.com/en
France
Owner of the Declaration
ONDULINE SA +33 1 55 63 80 10
Quai Gallieni 24 info@onduline.fr
92150 SURESNES www.onduline.com
France
12 Environmental Product Declaration - ONDULINE SA - Corrugated bitumen sheets and tiles for roofing application
