ENVIRONMENTAL PRODUCT DECLARATION
as per ISO 14025 and EN 15804+A2
Owner of the Declaration VELUX Group
Publisher Institut Bauen und Umwelt e.V. (IBU)
Programme holder Institut Bauen und Umwelt e.V. (IBU)
Declaration number EPD-VEL-20220113-CBB3-EN
Issue date 24/05/2022
Valid to 23/05/2027
VELUX flashings for profiled roofing material
VELUX Group
www.ibu-epd.com | https://epd-online.com
General Information
VELUX Group VELUX flashings for profiled roofing material
Programme holder Owner of the declaration
IBU – Institut Bauen und Umwelt e.V. VELUX Group
Hegelplatz 1 Ådalsvej 99
10117 Berlin 2970 Hørsholm
Germany Denmark
Declaration number Declared product / declared unit
EPD-VEL-20220113-CBB3-EN 1m² flashing for profiled roofing material EDW
The declared unit is based on the configuration of a standard size window
measuring 0.78m x 1.178m.
This declaration is based on the product category rules: Scope:
Windows and doors , 01/08/2021 Productline EDW - Flashing; manufactured by VELUX in France, Hungary,
(PCR checked and approved by the SVR) Poland, Denmark and China for sale in Europe.
Issue date Declaration according to ISO 14025 and EN 15804 describing specific
environmental performances of the construction product.
24/05/2022
The owner of the declaration shall be liable for the underlying information
and evidence; the IBU shall not be liable with respect to manufacturer
information, life cycle assessment data and evidences.
Valid to
23/05/2027 The EPD was created according to the specifications of EN 15804+A2. In
the following, the standard will be simplified as EN 15804.
Verification
The standard EN 15804 serves as the core PCR
Independent verification of the declaration and data according to ISO
14025:2011
internally X externally
Dipl.-Ing. Hans Peters
(Chairman of Institut Bauen und Umwelt e.V.)
Florian Pronold Prof. Dr. Birgit Grahl,
(Managing Director Institut Bauen und Umwelt e.V.) (Independent verifier)
1 Environmental Product Declaration - VELUX Group - VELUX flashings for profiled roofing material
Product
Product description/Product definition
The VELUX flashings for profiled roofing material are products REACH
for sale in the European market. This group of flashings cover a
large range of different flashing types for profiled roofing This product/article/at least one partial article contains
material. substances listed in the candidate list (date: 17.01.2022)
exceeding 0.1 percentage by mass: no.
The different flashing types fit for installation with either a single
window configuration or configurations of multiple windows Recycled content
installed adjacent to each other. All the flashings consist mainly
of aluminium.
The calculations are based on the representative flashing for
profiled roofing material named EDW. In the LCA, the EDW was
assessed to be a conservative choice for a representative
flashing for profiled roofing material type. For the use and The values stated in the table relate to the recycled material
application of the product the respective national provisions at streams in VELUX production.
the place of use apply, in Germany for example the building
codes of the federal states and the corresponding national Reference service life
specifications. A calculation of the reference service life according to ISO
15686 is not possible.
Application
VELUX flashings for profiled roofing material are used in The Bundesinstitut für Bau, Stadt und Raumforschung/Federal
renovation and new build. Either installed as a single window or office for building and regional planning (BBSR)
in a combination of multiple windows. table declares for the complete roof window a service life
dependent on the applied window frame material between 25
Technical Data
and ≥ 50 years. This includes collars and flashings as declared
The performance values are specific for the EDW flashing.
with this EPD.
The declared values in the table relate to the reference product.
Constructional data
Name Value Unit
Reaction to fire EN 13501-1 E class
Performance data of the product with respect to its
characteristics in accordance with the relevant technical
provision (no CE-marking).
Base materials/Ancillary materials
Name Value Unit
Aluminium 57% %
Galvanized steel 1 %
Stainless steel 0.3 %
Polybutadiene 35 %
EPDM 2 %
Polyethylene LD 2 %
Hot-melt adhesive 1 %
Silicone 1 %
LCA: Calculation rules
Declared Unit System boundary
The declared unit is one m² related to a reference window, that Type of EPD: Cradle to gate - with options. The following life
the flashing is installed in connection with. cycle stages were considered:
The declared unit is based on the representative product Production stage A1-A3:
measuring 0.78m x 1.178m. Consideration of the production of raw materials and their
processing; transport of major material to the manufacturing
Declared unit
site; assembly of semi-finished products to the final product;
Name Value Unit
packaging material (including waste paper input for paper and
Declared unit 1 m2 cardboard).
Weight per area 4.77 kg/representative product
End-of-Life stage C1, C2, C3:
Weight per area 5.18 kg/declared unit
2 Environmental Product Declaration - VELUX Group - VELUX flashings for profiled roofing material
C1: a manual demolition is assumed, resulting in indicator value
"0". Contribution of waste flows is considered in the modules where
C2: For the transport to EoL by truck a distance of 50 km is they occur.
assumed.
C3: A scenario for the incineration of plastics in a waste Geographic Representativeness
incineration plant (WIP) is assumed. Land or region, in which the declared product system is
manufactured, used or handled at the end of the product´s
The EoL-Scenario does not assume waste to be disposed of on lifespan: Europe
a landfill site. Module C4 is declared as "0".
Comparability
Benefits for the next product system D:
Basically, a comparison or an evaluation of EPD data is only
Resulting electrical and thermal energy from the WIP, avoiding
possible if all the data sets to be compared were created
the generation of electricity and heat via fossil fuels, is
according to EN 15804 and the building context, respectively
considered.
the product-specific characteristics of performance, are taken
The amount of metals after the reduction due to the net-flow
into account. The software GaBi is used accompanied by the
calculations is sent to a recycling process. The effort for
GaBi background data base (version 2021.2, 2021).
recycling, as well as the benefit for the regained metals are
declared in module D.
LCA: Scenarios and additional technical information
Characteristic product properties of biogenic carbon
The following declared values refer to the declared unit of 1m².
Information on describing the biogenic Carbon Content at
factory gate Reference service life
The declared biogenic content comprises the paper manual Name Value Unit
and the packaging material consisting of cardboard, paper and
Life Span (according to BBSR) depending on 25 -
wood. As module A5 is not declared, the information on a
window frame material 50
packaging supports further EoL calculations.
Name ValueUnit End of life (C1-C4)
kg Name Value Unit
Biogenic carbon content in product -
C Collected separately waste type waste type 5.18 kg
Biogenic carbon content in accompanying 0.592 kg Recycling 3.03 kg
packaging C
Energy recovery 2.13 kg
The value refers to the following packaging material (per 1m²):
Paper (manual): 0.024kg, Cardboard packaging: 1.347kg, Reuse, recovery and/or recycling potentials (D), relevant
Paper insert: 0.007kg, PE-LD: 0.008kg scenario information
Name Value Unit
Note: 1 kg of biogenic carbon is equivalent to 44/12 kg of CO .
2 Aluminium (net-flow calculation) 1.96 kg/1m² product
Steel (net-flow calculation) 0.09 kg/1m² product
Stainless steel (net-flow calculation) 8.18E-03 kg/1m² product
3 Environmental Product Declaration - VELUX Group - VELUX flashings for profiled roofing material
LCA: Results
DESCRIPTION OF THE SYSTEM BOUNDARY (X = INCLUDED IN LCA; MND = MODULE OR INDICATOR NOT DECLARED; MNR
= MODULE NOT RELEVANT)
Benefits and
Construction loads beyond
Product stage Use stage End of life stage
process stage the system
boundaries
la ire ta m w a Ry lp p u s tro p s n a rT g n iru tc a fu n a M e h t m o rf tro p s n a rTe tis e h t o t e ta g y lb m e s s A e s U e c n a n e tn ia M ria p e R tn e m e c a lp e R tn e m h s ib ru fe R y g re n e la n o ita re p Oe s u re ta w la n o ita re p Oe s u n o itc u rts n o c -e Dn o itilo m e d tro p s n a rT g n is s e c o rp e ts a W la s o p s iD -e s u e R-y re v o c e R-g n ilc y c e Rla itn e to p
A1 A2 A3 A4 A5 B1 B2 B3 B4 B5 B6 B7 C1 C2 C3 C4 D
X X X MND MND MND MND MNR MNR MNR MND MND X X X X X
RESULTS OF THE LCA - ENVIRONMENTAL IMPACT according to EN 15804+A2: 1 m² EDW
Parameter Unit A1-A3 C1 C2 C3 C4 D
Global Warming Potential total (GWP-total) kg CO 2 eq 2.88E+01 0 1.58E-02 7.21E+00 0 -1.76E+01
Global Warming Potential fossil fuels (GWP-fossil) kg CO 2 eq 3.09E+01 0 1.57E-02 7.21E+00 0 -1.75E+01
Global Warming Potential biogenic (GWP-biogenic) kg CO 2 eq -2.14E+00 0 -1.86E-05 2.86E-04 0 -5.15E-02
Global Warming Potential luluc (GWP-luluc) kg CO 2 eq 1.7E-02 0 1.28E-04 9.47E-05 0 -7.35E-03
Depletion potential of the stratospheric ozone layer (ODP) kg CFC11 eq 2.44E-11 0 3.09E-18 9.31E-16 0 -5.13E-14
Acidification potential of land and water (AP) mol H+ eq 1.22E-01 0 3.09E-05 7.36E-04 0 -7.63E-02
Eutrophication potential aquatic freshwater (EP-freshwater) kg P eq 1.76E-04 0 4.65E-08 1.36E-07 0 -9.77E-06
Eutrophication potential aquatic marine (EP-marine) kg N eq 2.01E-02 0 1.28E-05 1.71E-04 0 -1.04E-02
Eutrophication potential terrestrial (EP-terrestrial) mol N eq 2.14E-01 0 1.45E-04 3.42E-03 0 -1.13E-01
Formation potential of tropospheric ozone photochemical oxidants kg NMVOC
9.44E-02 0 2.76E-05 5.01E-04 0 -3.19E-02
(POCP) eq
Abiotic depletion potential for non fossil resources (ADPE) kg Sb eq 1.58E-05 0 1.39E-09 1.37E-08 0 -2.31E-06
Abiotic depletion potential for fossil resources (ADPF) MJ 5.41E+02 0 2.08E-01 1.32E+00 0 -2.37E+02
m3 world eq
Water use (WDP) 1.06E+01 0 1.45E-04 6.54E-01 0 -2.83E+00
deprived
RESULTS OF THE LCA - INDICATORS TO DESCRIBE RESOURCE USE according to EN 15804+A2: 1 m² EDW
Parameter Unit A1-A3 C1 C2 C3 C4 D
Renewable primary energy as energy carrier (PERE) MJ 1.22E+02 0 1.2E-02 2.75E-01 0 -9.63E+01
Renewable primary energy resources as material utilization
MJ 2.2E+01 0 0 0 0 0
(PERM)
Total use of renewable primary energy resources (PERT) MJ 1.44E+02 0 1.2E-02 2.75E-01 0 -9.63E+01
Non renewable primary energy as energy carrier (PENRE) MJ 4.5E+02 0 2.09E-01 9.33E+01 0 -2.37E+02
Non renewable primary energy as material utilization (PENRM) MJ 9.2E+01 0 0 -9.2E+01 0 0
Total use of non renewable primary energy resources (PENRT) MJ 5.42E+02 0 2.09E-01 1.33E+00 0 -2.37E+02
Use of secondary material (SM) kg 2.39E+00 0 0 0 0 1.9E+00
Use of renewable secondary fuels (RSF) MJ 0 0 0 0 0 0
Use of non renewable secondary fuels (NRSF) MJ 0 0 0 0 0 0
Use of net fresh water (FW) m3 4.62E-01 0 1.37E-05 1.54E-02 0 -2.36E-01
RESULTS OF THE LCA – WASTE CATEGORIES AND OUTPUT FLOWS according to EN 15804+A2:
1 m² EDW
Parameter Unit A1-A3 C1 C2 C3 C4 D
Hazardous waste disposed (HWD) kg 5.27E-07 0 1.1E-11 2.37E-10 0 -4.8E-06
Non hazardous waste disposed (NHWD) kg 5.35E+00 0 3.28E-05 1.89E-01 0 -4.3E+00
Radioactive waste disposed (RWD) kg 2.31E-02 0 3.79E-07 6.31E-05 0 -1.49E-02
Components for re-use (CRU) kg 0 0 0 0 0 0
Materials for recycling (MFR) kg 0 0 0 2.8E+00 0 0
Materials for energy recovery (MER) kg 0 0 0 0 0 0
Exported electrical energy (EEE) MJ 0 0 0 1.46E+01 0 0
Exported thermal energy (EET) MJ 0 0 0 2.61E+01 0 0
RESULTS OF THE LCA – additional impact categories according to EN 15804+A2-optional:
1 m² EDW
Parameter Unit A1-A3 C1 C2 C3 C4 D
Disease
Incidence of disease due to PM emissions (PM) 1.25E-06 0 1.87E-10 6.18E-09 0 -7.97E-07
incidence
Human exposure efficiency relative to U235 (IR) kBq U235 eq 4.48E+00 0 5.55E-05 9.28E-03 0 -2.94E+00
Comparative toxic unit for ecosystems (ETP-fw) CTUe 4.13E+02 0 1.55E-01 7.77E-01 0 -7.76E+01
Comparative toxic unit for humans (carcinogenic) (HTP-c) CTUh 4.23E-08 0 3.13E-12 5.89E-11 0 -9.68E-09
4 Environmental Product Declaration - VELUX Group - VELUX flashings for profiled roofing material
Comparative toxic unit for humans (noncarcinogenic) (HTP-nc) CTUh 5.75E-07 0 1.7E-10 3.88E-09 0 -1.98E-07
Soil quality index (SQP) SQP 1.71E+02 0 7.16E-02 3.46E-01 0 -1.43E+01
Disclaimer 1 – for the indicator 'Potential Human exposure efficiency relative to U235'.
This impact category deals mainly with the eventual impact of low dose ionizing radiation on human health of the nuclear fuel cycle. It
does not consider effects due to possible nuclear accidents, occupational exposure or radioactive waste disposal in underground
facilities. Potential ionizing radiation from the soil, radon and from some construction materials is also not measured by this indicator.
Disclaimer 2 – for the indicators 'abiotic depletion potential for non-fossil resources', 'abiotic depletion potential for fossil resources',
'water (user) deprivation potential, deprivation-weighted water consumption', 'potential comparative toxic unit for ecosystems', 'potential
comparative toxic unit for humans – cancerogenic', 'Potential comparative toxic unit for humans - not cancerogenic', 'potential soil
quality index'. The results of this environmental impact indicator shall be used with care as the uncertainties on these results are high
or as there is limited experience with the indicator.
Disclaimer 3 – for 'potential soil quality index'. Due to a data lack in the foreground data of VELUX, the result has a very high
uncertainty and refers only to the background data, which contain respective information.
References
BBSR EN ISO 14025:2011, Environmental labels and declarations —
BBSR, 24.02.2017, Nutzungsdauer von Bauteilen nach BNB Type III environmental declarations — Principles and
procedures.
DIN EN 13501
DIN EN 13501-1:2019-05: Fire classification of construction ISO 15686
products and building elements - Part 1: Classification using ISO 15686:2011-05: Buildings and constructed assets - Service
data from reaction to fire tests life planning - Part 1: General principles and framework
DIN EN ISO 10077 PCR part A
DIN EN ISO 10077-1:2020-10: Thermal performance of Calculation Rules for the Life Cycle Assessment and
windows, doors and shutters - Calculation of thermal Requirements on the Project Report according to EN
transmittance 15804+A2:2019, version 1.2, Berlin: Institut Bauen und Umwelt
e.V., 2021
EN 15804
EN 15804:2012+A2:2019, Sustainability of construction works PCR part B
— Environmental Product Declarations — Core rules for the Requirements on the EPDS for Windows and doors, version
product category of construction products. 01-2021, Berlin: Institut Bauen und Umwelt e.V.
GaBi REACH
GaBi Software and GaBi Database by Sphera Solution GmbH, Regulation (EC) No 1907/2006 of the European Parliament and
version: 2021.2, 2021 of the Council on the Registration, Evaluation, Authorisation
and Restriction of Chemicals (REACH)
IBU 2021
Institut Bauen und Umwelt e.V.: General Instructions for the Regulation (EU) No. 305/2011 (CPR)
EPD programme of Institut Bauen und Umwelt e.V., Version Regulation (EU) No 305/2011 of the European Parliament and
2.0, Berlin: Institut Bauen und Umwelt e.V., 2021, www.ibu- of the Council of 9 March 2011 laying down harmonized
epd.com conditions for the marketing of construction products and
repealingCounsicl Directive 89/106/EEC
ISO 14025
5 Environmental Product Declaration - VELUX Group - VELUX flashings for profiled roofing material
Publisher
Institut Bauen und Umwelt e.V. +49 (0)30 3087748- 0
Hegelplatz 1 info@ibu-epd.com
10117 Berlin www.ibu-epd.com
Germany
Programme holder
Institut Bauen und Umwelt e.V. +49 (0)30 3087748- 0
Hegelplatz 1 info@ibu-epd.com
10117 Berlin www.ibu-epd.com
Germany
Author of the Life Cycle Assessment
Daxner & Merl GmbH +43 676 849477826
Lindengasse 39/8 office@daxner-merl.com
1070 Wien www.daxner-merl.com
Austria
Angela Schindler Umweltberatung 07553 919 9456
Tüfinger Str. 12 angela@schindler-umwelt.de
88682 Salem www.schindler-umwelt.de
Germany
Owner of the Declaration
VELUX Group +4545164726
Ådalsvej 99 jakob.roerbech@velux.com
2970 Hørsholm www.velux.com
Denmark
6 Environmental Product Declaration - VELUX Group - VELUX flashings for profiled roofing material
