ENVIRONMENTAL PRODUCT DECLARATION
as per ISO 14025 and EN 15804+A2
Owner of the Declaration Liapor
Publisher Institut Bauen und Umwelt e.V. (IBU)
Programme holder Institut Bauen und Umwelt e.V. (IBU)
Declaration number EPD-LIA-20230117-CCC1-EN
Issue date 13.07.2023
Valid to 12.07.2028
Lightweight expanded clay aggregate for loose-fill applications
Liapor
www.ibu-epd.com | https://epd-online.com
General Information
Liapor Lightweight expanded clay aggregate for loose-fill
applications
Programme holder Owner of the declaration
IBU – Institut Bauen und Umwelt e.V. Liapor
Hegelplatz 1 Industriestr 2
10117 Berlin 91352 Hallerndorf
Germany Germany
Declaration number Declared product / declared unit
EPD-LIA-20230117-CCC1-EN 1 ton of lightweight expanded clay aggregates use in loose fill applications
This declaration is based on the product category rules: Scope:
Lightweight aggregates / Bulk granulate, 01.08.2021 This EPD refers to the lightweight expanded clay aggregate from Liapor
(PCR checked and approved by the SVR) GmbH & Co used in different thermal insulation applications for buildings
(EN 14063-1) or lightweight fill applications in civil engineering works (EN
15732).
Issue date The commercial references covered by this EPD are the following: Liapor
2.9E, Liapor 2B, Liapor 3, and Liapor G3. These products are
13.07.2023
manufactured in the Liapor factory in Pautzfeld, Germany.
The owner of the declaration shall be liable for the underlying information
and evidence; the IBU shall not be liable with respect to manufacturer
Valid to
information, life cycle assessment data and evidences.
12.07.2028
The EPD was created according to the specifications of EN 15804+A2. In
the following, the standard will be simplified as EN 15804.
Verification
The standard EN 15804 serves as the core PCR
Independent verification of the declaration and data according to ISO
14025:2011
internally X externally
Dipl.-Ing. Hans Peters
(Chairman of Institut Bauen und Umwelt e.V.)
Florian Pronold Mr Olivier Muller,
(Managing Director Institut Bauen und Umwelt e.V.) (Independent verifier)
1 Environmental Product Declaration - Liapor - Lightweight expanded clay aggregate for loose-fill applications
Product
(https://www.liapor.com/en/products/declaration-of-
Product description/Product definition performance.html).
Lightweight expanded clay aggregate is made from clay. The
Constructional data
raw lias clay is crushed, ground dry to flour and then granulated
into small balls by adding water. These are then heated to Name Value Unit
around 1,200 °C in a rotary kiln, where their volume increases. Loose bulk density 235 - 350 kg/m3
The manufacturing process is completed by firing the expanded Particle size 2 - 16 mm
balls. This process enables the size, weight and strength of the
Crushing resistance 0.45 - 1.25 MPa
Liapor granules to be precisely controlled.
Water absorption W24h 14 - 26 M %
Performance data of the product in accordance with the
declaration of performance with respect to its essential
characteristics according to EN 15804:2019+A2, Sustainability
of construction works - Environmental product declarations –
Core rules for the product category of construction products.
The product has a long life span and does not require
maintenance. When the product is used in structural concrete, it
Voluntary data: Draft for Product Category Rules (c-PCR)
can reduce the weight of concrete by almost 50 % without
complementary to EN 16783 for unbounded expanded clay
compromising strength. Lightweight expanded clay aggregate
aggregates, 2021.
is lighter than loose gravel or loose-fill crushed stone and can
sustain dynamic loads. Besides, the product in loose-fill Base materials/Ancillary materials
applications is reusable at 75 %, and it is classified as a fully
Composition of lightweight expanded clay aggregate
non-combustible material (A1 Euroclass).
In the present EPD, only loose-fill applications are considered. Name Value Unit
Clay > 98 M.-%
Application
Additives < 2 M.-%
It can be used in different applications such as structural
concrete, precast concrete, concrete blocks, thermal insulation This product does not contain substances from the "Candidate
(EN 14063-1) and geotechnical lightweight fill applications (EN List of Substances of Very High Concern for Authorisation".
15732).
Reference service life
This EPD only includes use in loose-fill applications.
The RSL of expanded clay aggregates is usually 100 years. If
Technical Data the building lifespan is 50 years, a scenario of reuse can be
Lightweight expanded clay aggregates follow EN 14063-1 for retained for the expanded clay aggregates at its end of life,
thermal insulation and EN 15732 for geotechnical lightweight fill depending on whether the product is clean or contaminated.
applications. The product is classified as a fully non- This reuse can take place on the same site or at another
combustible material (A1 Euroclass). location.
For more information, look at their Declaration of Performance
LCA: Calculation rules
Declared Unit System boundary
This EPD provides results based on the declared unit defined The whole life cycle is considered for the lightweight expanded
for the product applied in lightweight fillings and thermal clay aggregate in the scope of this EPD.
insulation. The final product follows the EN 15732 standard for The lightweight expanded clay aggregates are composed
lightweight filling in civil engineering works. For thermal mainly of clay and limestone. They are extracted and then
insulation, the final product transported to the factory, all transport is mass-based. The
follows the EN 16783 standard. Based on the declared unit in manufacturing of expanded clay aggregates is mainly in the
this EPD, the results are cradle-to-grave. kiln.
The declared unit defined is 1 ton of expanded clay lightweight
aggregates, representing 3.048 m3 (with a loose bulk density of Geographic Representativeness
328 kg/m3). Land or region, in which the declared product system is
manufactured, used or handled at the end of the product´s
Declared unit and mass reference
lifespan: Germany
Name Value Unit
Loose bult density 328 kg/m3
Comparability
Declared unit 3.048 m3
Basically, a comparison or an evaluation of EPD data is only
possible if all the data sets to be compared were created
The EPD is specific to one company and one type of product. according to EN 15804 and the building context, respectively
Aspects regarding average EPDs are not applicable. the product-specific characteristics of performance, are taken
into account.
LCA: Scenarios and additional technical information
2 Environmental Product Declaration - Liapor - Lightweight expanded clay aggregate for loose-fill applications
Reference service life
Characteristic product properties of biogenic carbon
Lightweight expanded clay aggregates are mainly made from Name Value Unit
clay without biogenic carbon content. Thus, no additional Reference service life (according to ISO
100 a
calculation for global warming potential excluding or including 15686-1, -2, -7 and -8)
biogenic CO₂ emissions is provided. EN 15732
Declared product properties (at the gate)
and EN -
and finishes
The products covered by this EPD are described as follows, 14063-1
according to their Declaration of Performance
Design application parameters (if instructed
(https://www.liapor.com/en/products/declaration-of- EN 15732
by the manufacturer), including the
performance.html): and EN -
references to the appropriate practices and
14063-1
• Liapor 2.9E: round, 2-6 mm, 290+/- 25 kg/m3 application codes
• Liapor 2B: round, 4-10 mm, 235+/- 25 kg/m3 An assumed quality of work, when installed EN 15732
• Liapor 3: round, 4-8 mm, 325+/- 25 kg/m3 in accordance with the manufacturer’s and EN -
• Liapor G3: round, 4-16 mm, 325+/- 25 kg/m3 instructions 14063-1
Outdoor environment, (for outdoor
applications), e.g. weathering, pollutants, Not
Transport to the building site (A4) -
UV and wind exposure, building orientation, applicable
Name Value Unit
shading, temperature
Litres of fuel - l/100km
Indoor environment (for indoor
Not
Transport distance 420 km applications), e.g. temperature, moisture, -
applicable
Capacity utilisation (including empty runs) 53 % chemical exposure
Loose bulk density of product transported 290 - 325 kg/m3 Usage conditions, e.g. frequency of use, Not
-
Capacity utilisation volume factor - - mechanical exposure applicable
Maintenance e.g. required frequency, type
Not
Installation into the building (A5) and quality and replacement of -
applicable
Name Value Unit components
Other resources Diesel consumption 0.44 kg
End of life (C1 - C4)
25% of the product is landfilled, and 75% is reused without the
The reference service lifetime of building products is a factor of need for any other treatment. The landfilled product is
high uncertainty. According to expert judgments, the information transported by truck to an inert landfill
on the lifespan of expanded clay aggregates is 100 years, as
Name Value Unit
installed products are still in use.
Collected separately waste type 1000 kg
Liapor expanded clay aggregates are already installed in
existing buildings and construction works in previous decades Collected as mixed construction waste - kg
(product intrinsic material properties lead to good long-term Reuse 750 kg
performances). If installed correctly according to the Recycling - kg
manufacturer's guidelines, the expanded clay aggregates need
Energy recovery - kg
no further maintenance, repair, replacement, or refurbishment
Landfilling 250 kg
during the full life span of the product.
3 Environmental Product Declaration - Liapor - Lightweight expanded clay aggregate for loose-fill applications
LCA: Results
The whole life cycle is considered for the lightweight expanded clay aggregate in the scope of this EPD. The system boundaries
correspond to the diagram provided in Table 1 in line with the requirements of EN 15804 A2. Within this standard, the life cycle stages
and processes are structured in a modular system (modules A-D) as follows:
• Modules A1-3 = production stage:covers raw material
supply (A1), transport of raw materials (A2)
andmanufacturing (A3),
• Modules A4–5 = construction stage:covers transport to
the construction site (A4) and
construction/installationprocesses (A5),
• Module B1-7 = use stage: covers use(B1), maintenance
(B2), repair (B3), replacement (B4), refurbishment
(B5),operational energy use (B6) and operational water
use (B7),
• Modules C1-4 = end-of-life: coversde-
construction/demolition (C1), transport (C2), waste
processing (C3) anddisposal (C4),
• Module D = includes the benefits and loads beyond the
system.
DESCRIPTION OF THE SYSTEM BOUNDARY (X = INCLUDED IN LCA; ND = MODULE OR INDICATOR NOT DECLARED; MNR =
MODULE NOT RELEVANT)
Benefits and
Construction loads beyond
Product stage Use stage End-of-life stage
process stage the system
boundaries
la ire ta m w a Ry lp p u s tro p s n a rT g n iru tc a fu n a M e h t m o rf tro p s n a rTe tis e h t o t e ta g y lb m e s s A e s U e c n a n e tn ia M ria p e R tn e m e c a lp e R tn e m h s ib ru fe R y g re n e la n o ita re p Oe s u re ta w la n o ita re p Oe s u n o itc u rts n o c -e Dn o itilo m e d tro p s n a rT g n is s e c o rp e ts a W la s o p s iD -e s u e R-y re v o c e R-g n ilc y c e Rla itn e to p
A1 A2 A3 A4 A5 B1 B2 B3 B4 B5 B6 B7 C1 C2 C3 C4 D
X X X X X X X X X X X MND X X X X X
RESULTS OF THE LCA - ENVIRONMENTAL IMPACT according to EN 15804+A2: 1 ton lightweight expanded clay aggregates
Parameter Unit A1 A2 A3 A4 A5 B1 B2 B3 B4 B5 B6 C1 C2 C3 C4 D
GWP-total kg CO 2 2.22E 9.73E-01 4.83E 5.1E+01 7.67E-01 0 0 0 0 0 0 8.44E-02 1.52E 0 3.63E -3.62E
eq +00 +02 +00 +00 +02
GWP-fossil kg CO 2 2.22E 9.69E-01 4.88E 5.08E 8.3E-01 0 0 0 0 0 0 1.19E-01 1.51E 0 3.73E -3.66E
eq +00 +02 +01 +00 +00 +02
GWP- kg CO 2 -6.03E- 3.98E-04 -4.38E -6.99E- -6.93E- 0 0 0 0 0 0 -3.78E- -2.08E- 0 -1.11E- 3.28E
biogenic eq 04 +00 02 02 02 03 01 +00
GWP-luluc kg CO 2 1.48E-033.61E-031.82E-022.82E-01 5.88E-03 0 0 0 0 0 0 3.19E-03 8.39E-03 0 6.89E-03 -2.38E-
eq 03
kg CFC11 -3.41E-
ODP 1.24E-121.38E-134.54E-093.03E-12 3.33E-13 0 0 0 0 0 0 1.22E-13 9.02E-14 0 8.77E-12
eq 09
2.07E -1.55E
AP mol H+ eq 6.19E-033.19E-03 1.71E-01 8.73E-04 0 0 0 0 0 0 4.29E-04 5.08E-03 0 2.65E-02
+00 +00
EP- -2.43E-
kg P eq 2.43E-06 2E-06 3.87E-051.51E-04 3.28E-06 0 0 0 0 0 0 1.77E-06 4.49E-06 0 6.33E-06
freshwater 05
-1.47E-
EP-marine kg N eq 1.42E-03 1.5E-03 1.99E-017.93E-02 1.71E-04 0 0 0 0 0 0 7.95E-05 2.36E-03 0 6.77E-03
01
4 Environmental Product Declaration - Liapor - Lightweight expanded clay aggregate for loose-fill applications
2.17E -1.61E
EP-terrestrial mol N eq 1.54E-021.68E-02 8.86E-01 2.41E-03 0 0 0 0 0 0 1.1E-03 2.64E-02 0 7.43E-02
+00 +00
kg
POCP NMVOC 5.06E-032.88E-03 6.7E-01 1.54E-01 6.58E-04 0 0 0 0 0 0 3.21E-04 4.59E-03 0 2.06E-02 -5E-01
eq
-2.81E-
ADPE kg Sb eq 1E-07 1.05E-064.23E-06 1.65E-07 0 0 0 0 0 0 8.84E-08 1.26E-07 0 3.82E-07 1.47E-06
06
2.42E 1.29E 2.06E 6.76E 1.14E 2.01E 4.89E -1.54E
ADPF MJ 2.11E+01 0 0 0 0 0 0 0
+01 +01 +03 +02 +01 +01 +01 +03
m3 world
-2.45E- 3.54E -2.63E
WDP eq 3.81E-03 4.54E-01 6.4E-02 0 0 0 0 0 0 3.37E-03 1.35E-02 0 4.09E-01
03 +00 +00
deprived
GWP = Global warming potential; ODP = Depletion potential of the stratospheric ozone layer; AP = Acidification potential of land and water; EP =
Eutrophication potential; POCP = Formation potential of tropospheric ozone photochemical oxidants; ADPE = Abiotic depletion potential for non-fossil
resources; ADPF = Abiotic depletion potential for fossil resources; WDP = Water (user) deprivation potential)
RESULTS OF THE LCA - INDICATORS TO DESCRIBE RESOURCE USE according to EN 15804+A2: 1 ton lightweight expanded
clay aggregates
Parameter Unit A1 A2 A3 A4 A5 B1 B2 B3 B4 B5 B6 C1 C2 C3 C4 D
3.16E 6.03E 3.84E 1.14E 7.33E -4.61E
PERE MJ 7.65E-01 1.3E+00 0 0 0 0 0 0 6.76E-01 0
+00 +01 +01 +00 +00 +01
PERM MJ 0 0 0 0 0 0 0 0 0 0 0 0 0 0 0 0
3.16E 6.03E 3.84E 1.14E 7.33E -4.61E
PERT MJ 7.65E-01 1.3E+00 0 0 0 0 0 0 6.76E-01 0
+00 +01 +01 +00 +00 +01
2.42E 1.29E 2.06E 6.78E 2.12E 1.14E 2.02E 4.89E -1.54E
PENRE MJ 0 0 0 0 0 0 0
+01 +01 +03 +02 +01 +01 +01 +01 +03
1.16E -1.16E
PENRM MJ 0 0 0 0 0 0 0 0 0 0 0 0 0 0
+01 +01
2.42E 1.29E 2.07E 6.78E 9.56E 1.14E 2.02E 4.89E -1.54E
PENRT MJ 0 0 0 0 0 0 0
+01 +01 +03 +02 +00 +01 +01 +01 +03
SM kg 0 0 0 0 0 0 0 0 0 0 0 0 0 0 0 0
RSF MJ 0 0 0 0 0 0 0 0 0 0 0 0 0 0 0 0
NRSF MJ 0 0 0 0 0 0 0 0 0 0 0 0 0 0 0 0
FW m3 9.35E-011.21E-036.67E-048.71E-014.35E-02 0 0 0 0 0 0 5.89E-041.29E-03 0 1.24E-02-6.52E-01
PERE = Use of renewable primary energy excluding renewable primary energy resources used as raw materials; PERM = Use of renewable primary
energy resources used as raw materials; PERT = Total use of renewable primary energy resources; PENRE = Use of non-renewable primary energy
excluding non-renewable primary energy resources used as raw materials; PENRM = Use of non-renewable primary energy resources used as raw
materials; PENRT = Total use of non-renewable primary energy resources; SM = Use of secondary material; RSF = Use of renewable secondary fuels;
NRSF = Use of non-renewable secondary fuels; FW = Use of net fresh water
RESULTS OF THE LCA – WASTE CATEGORIES AND OUTPUT FLOWS according to EN 15804+A2:
1 ton lightweight expanded clay aggregates
Parameter Unit A1 A2 A3 A4 A5 B1 B2 B3 B4 B5 B6 C1 C2 C3 C4 D
HWD kg 4.74E-08 3.8E-08 5.95E-11 3.14E-093.24E-09 0 0 0 0 0 0 5.26E-11 9.65E-11 0 2.51E-09-3.07E-08
2.69E -1.37E
NHWD kg 3.58E-012.04E-03 1.8E+01 9.71E-02 0 0 0 0 0 0 1.8E-03 2.89E-03 0 2.5E+02
+02 +01
RWD kg 8.3E-02 6.12E-05 1.3E-05 8.15E-028.35E-04 0 0 0 0 0 0 1.14E-052.48E-05 0 5.44E-04-6.11E-02
7.5E
CRU kg 0 0 0 0 0 0 0 0 0 0 0 0 0 0 0
+02
MFR kg 0 0 0 0 0 0 0 0 0 0 0 0 0 0 0 0
MER kg 0 0 0 0 0 0 0 0 0 0 0 0 0 0 0 0
EEE MJ 0 0 0 0 0 0 0 0 0 0 0 0 0 0 0 0
EET MJ 0 0 0 0 0 0 0 0 0 0 0 0 0 0 0 0
HWD = Hazardous waste disposed; NHWD = Non-hazardous waste disposed; RWD = Radioactive waste disposed; CRU = Components for re-use;
MFR = Materials for recycling; MER = Materials for energy recovery; EEE = Exported electrical energy; EET = Exported thermal energy
RESULTS OF THE LCA – additional impact categories according to EN 15804+A2-optional:
1 ton lightweight expanded clay aggregates
Parameter Unit A1 A2 A3 A4 A5 B1 B2 B3 B4 B5 B6 C1 C2 C3 C4 D
Disease
PM 2.27E-07 1.7E-08 1.58E-059.08E-076.96E-09 0 0 0 0 0 0 3.26E-09 2.7E-08 0 3.26E-07 -1.2E-05
incidence
kBq U235 2.62E -1.97E
IR 9.22E-021.26E-03 1.22E-013.33E-03 0 0 0 0 0 0 1.11E-033.64E-03 0 6.03E-02
eq +01 +01
4.62E 1.02E 3.72E 4.69E 1.67E 9.01E 2.74E -2.65E
ETP-fw CTUe 0 0 0 0 0 0 1.4E+01 0
+00 +01 +02 +02 +01 +00 +01 +02
HTP-c CTUh 1.89E-102.03E-109.88E-099.46E-093.38E-10 0 0 0 0 0 0 1.79E-102.81E-10 0 4.18E-09 -7.2E-09
-1.08E-
HTP-nc CTUh 4.18E-081.15E-081.43E-065.62E-07 1.7E-08 0 0 0 0 0 0 8.77E-091.67E-08 0 4.63E-07
06
4.04E 3.53E 2.33E 6.63E 3.57E 6.92E 1.02E -1.98E
SQP SQP 3.6E+00 0 0 0 0 0 0 0
+00 +01 +02 +00 +00 +00 +01 +01
PM = Potential incidence of disease due to PM emissions; IR = Potential Human exposure efficiency relative to U235; ETP-fw = Potential comparative
Toxic Unit for ecosystems; HTP-c = Potential comparative Toxic Unit for humans (cancerogenic); HTP-nc = Potential comparative Toxic Unit for humans
(not cancerogenic); SQP = Potential soil quality index
Disclaimer 1 – for the indicator “Potential Human exposure efficiency relative to U235”. This impact category deals mainly with the
eventual impact of low-dose ionizing radiation on human health of the nuclear fuel cycle. It does not consider effects due to possible
5 Environmental Product Declaration - Liapor - Lightweight expanded clay aggregate for loose-fill applications
nuclear accidents, occupational exposure or radioactive waste disposal in underground facilities. Potential ionizing radiation from the
soil, radon and from some construction materials is also not measured by this indicator.
Disclaimer 2 – for the indicators “abiotic depletion potential for non-fossil resources”, “abiotic depletion potential for fossil resources”,
“water (user) deprivation potential, deprivation-weighted water consumption”, “potential comparative toxic unit for ecosystems”,
“potential comparative toxic unit for humans – cancerogenic”, “Potential comparative toxic unit for humans - not cancerogenic”,
“potential soil quality index”. The results of this environmental impact indicator shall be used with care as the uncertainties on these
results are high as there is limited experience with the indicator.
References
ISO 14025:2006 EN 14063-1:2004
ISO 14025:2006 Environmental labels and declarations — Type EN 14063-1 : Thermal insulation materials and products - In-
III environmental declarations — Principles and procedures situ formed expanded clay lightweight aggregate products
(LWA) - Part 1: Specification for the loose-fill products before
EN 15804 installation (+AC:2006)
EN 15804+A2:2019 Sustainability of construction works -
Environmental product declarations - Core rules for the product EN 15732
category of construction products EN 15732:2013 - Light weight fill and thermal insulation
products for civil engineering applications (CEA) - Expanded
PCR Part A: Calculation Rules for the Life Cycle Assessment clay lightweight aggregate products (LWA)
and Requirements on the Project Report according to EN
15804+A2:2019 (Institut für Bauen und Umwelt (IBU)) (v1.2), EN 16783
2021. EN 16783:2017 - Thermal insulation products - Product
category rules (PCR) for factory made and in-situ formed
PCR Part B: Requirements on the EPD (Institut für Bauen und products for preparing environmental product declarations
Umwelt (IBU)) (v1.7), 2019.
REACH Regulation
Software/Database Candidate List of Substances of Very High Concern for
Sphera LCA for Experts Authorisation
Sphera Database
6 Environmental Product Declaration - Liapor - Lightweight expanded clay aggregate for loose-fill applications
Publisher
Institut Bauen und Umwelt e.V. +49 (0)30 3087748- 0
Hegelplatz 1 info@ibu-epd.com
10117 Berlin www.ibu-epd.com
Germany
Programme holder
Institut Bauen und Umwelt e.V. +49 (0)30 3087748- 0
Hegelplatz 1 info@ibu-epd.com
10117 Berlin www.ibu-epd.com
Germany
Author of the Life Cycle Assessment
WeLOOP (+33) 9 81 85 76 82
Rue du Bourg 254 info@weloop.org
59130 Lambersart www.weloop.org
France
Owner of the Declaration
Liapor (+49) 95 45/4 48-0
Industriestr 2 info@liapor.com
91352 Hallerndorf www.liapor.ch
Germany
7 Environmental Product Declaration - Liapor - Lightweight expanded clay aggregate for loose-fill applications
