ver1 2015
ENVIRONMENTAL PRODUCT DECLARATION
in accordance with ISO 14025, ISO 21930 and EN 15804
Owner of the declaration: Helland Møbler AS
Program operator: The Norwegian EPD Foundation
Publisher: The Norwegian EPD Foundation
Declaration number: NEPD-3253-1894-EN
Registration number: NEPD-3253-1894-EN
ECO Platform reference number: -
Issue date: 22.11.2021
Valid to: 22.11.2026
Bo Dining table 180 x 90 cm
Helland Møbler AS
www.epd-norge.no
NEPD-3253-1894-EN Bo Dining table 180 x 90 cm
1 / 8
General information
Product: Owner of the declaration:
Bo Dining table 180 x 90 cm
Helland Møbler AS
Contact person: Joakim Helland
Phone: +47 958 09 013
e-mail: joakim.helland@helland.no
Program operator: Manufacturer:
Helland Møbler AS
The Norwegian EPD Foundation
Postboks 10 6259 Stordal
Pb. 5250 Majorstuen, 0303 Oslo
Norway
Phone: +47 23 08 80 00
e-mail: post@epd-norge.no
Declaration number: Place of production:
Helland Baltic ÖU
NEPD-3253-1894-EN Hapvali, Nõmme küla, Haapsalu linn EE-90439 Läänemaa
Estonia
ECO Platform reference number: Management system:
ISO 14001:2015, sertifikat nr 901085
This declaration is based on Product Category Rules: Organisation no:
943 511 128
CEN Standard EN 15804:2012+A1:2013 serves as core PCR
NPCR 026:2018 Part B for furniture
Statement of liability: Issue date: 22.11.2021
The owner of the declaration shall be liable for the underlying information and
evidence. EPD Norway shall not be liable with respect to manufacturer Valid to: 22.11.2026
information, life cycle assessment data and evidences.
Declared unit: Year of study:
1 Pcs Bo Dining table 180 x 90 cm 2020
Declared unit with option: Comparability:
A1,A2,A3,A4 EPDs from programmes other than the Norwegian EPD Foundation may not be
comparable
Functional unit: Development and verification of EPD:
Production of the table provided and maintained for a period of 15 years. The declaration has been developed and verified using EPD tool lca.tools
ver EPD2020.11, developed by LCA.no AS. The EPD tool is integrated into
the company's environmental management system, and has been
approved by EPD-Norway
General information on verification of EPD from EPD tools:
Independent verification of data, other environmental information and Developer of EPD:
the declaration according to ISO 14025:2010, § 8.1.3 and § 8.1.4. Individual
third party verification of each EPD is not required when the EPD tool is i) Oddrun Innselset
integrated into the company's environmental management system, ii) the
procedures for use of the EPD tool are approved by EPDNorway, and iii) Reviewer of company-specific input data and EPD:
the proccess is reviewed annualy. See Appendix G of EPD-Norway's
General Programme Instructions for further information on EPD tools. Pawel Sosinski
Verification of EPD tool: Approved:
Independent third party verification of the EPD tool, background data
Sign
and test-EPD in accordance with EPDNorway's procedures and guidelines
for verification and approval of EPD tools.
Erik Svanes, Norsus AS
(no signature required) Håkon Hauan, CEO EPD-Norge
Key environmental indicators Unit Cradle to gate A1 - A3
Global warming kg CO2 eqv 45,36
Total energy use MJ 1766,48
Amount of recycled materials % 10,11
NEPD-3253-1894-EN Bo Dining table 180 x 90 cm
2 / 8
Product
Market: Technical data:
Hight adjustsble
Europa and USA
Width: 180 cm
Product description: Height: 69,5-80 cm
Depth: 90 cm
Bo dining table base are supplied in natural birch, natural oak or using
standard range of stains. Table tops available
Reference service life, product
in imitation of oak, birch, white or light gray high-pressure laminate
with fitted edging. Other laminates on demand. 15 years
Can be delivered with hight-adjustable base: 69,5-80 cm. Table top
Reference service life, building
thickness 22 mm.
Product specification
Bo dining table base are supplied in natural birch, natural oak or using
standard range of stains. Table tops available
in imitation of oak, birch, white or light gray high-pressure laminate
with fitted edging. Other laminates on demand.
Can be delivered with hight-adjustable base: 69,5-80 cm. Table top
thickness 22 mm.
Recycled share in Recycled share in
Materials kg %
material (kg) material (%)
Metal - Steel 6,91 17,35 1,38 20,00
Wood - Solid beech/birch 5,71 14,33 0,00 0,00
Wood - Laminated wood 26,31 66,03 0,00 0,00
Paint, solvent-based 0,60 1,51 0,00 0,00
Plastic - Nylon (PA) 0,31 0,78 0,00 0,00
Total: 39,84 1,38
Recycled share in Recycled share in
Packaging kg
material (kg) material (%)
Packaging - Cardboard 4,00 3,05 76,30
Total including packaging 43,84 4,43
LCA: Calculation rules
Declared unit: Allocation:
The allocation is made in accordance with the provisions of EN 15804. Effects
1 Pcs Bo Dining table 180 x 90 cm
of primary production of recycled materials is allocated to the main product
Cut-off criteria: in which the material was used. The recycling process and transportation of
the material is allocated to this analysis.
All major raw materials and all the essential energy is included. The
production processes for raw materials and energy flows with very small
amounts (less than 1%) are not included. These cut-off criteria do not
apply for hazardous materials and substances.
Data quality:
Specific data for the product composition are provided by the manufacturer. They represent the production of the declared product and were collected for
EPD development in the year of study. Background data is based on registered EPDs according to EN 15804, Ostfold Research databases, ecoinvent and other
LCA databases. The data quality of the raw materials in A1 is presented in the table below.
Materials Source Data quality Year
Metal - Steel ecoinvent 3.3 Database 2016
Packaging - Cardboard ecoinvent 3.4 Database 2017
Paint, solvent-based ecoinvent 3.4 Database 2017
Wood - Laminated wood ecoinvent 3.4 Database 2017
Wood - Solid beech/birch ecoinvent 3.4 Database 2017
Plastic - Nylon (PA) ecoinvent 3.6 Database 2019
NEPD-3253-1894-EN Bo Dining table 180 x 90 cm
3 / 8
System boundary:
Additional technical information:
Transportation to an average customer in Copenhagen is 1000 km (A4: average European lorry > 32 tonnes)
The use stage (B1) is represented by a scenario and includes vacuum cleaning of textile once a month. The PCR does not
provide detailed guidelines for what should be included in the use stage. In the end of life stage, the transport distance for
waste to waste processing is 72 km (C1). The reuse, recovery and recycling stage is beyond the system boundaries (D). It is
assumed that the solution is dismantled and the materials recycled or combusted according to general Norwegian treatment of
industrial waste (see the table below). This calculation includes only CO2 emissions (GWP) in the C-modules. The transport
distance to reuse, recovery or recycling varies for each material, but the average distance is 373 km. The vehicles used and
associated data are described in detail in [5].
NEPD-3253-1894-EN Bo Dining table 180 x 90 cm
4 / 8
LCA: Scenarios and additional technical information
The following information describe the scenarios in the different modules of the EPD.
Transportation to an average customer in Copenhagen is 1000 km (A4: average European lorry > 32 tonnes) The use stage (B1) is represented by a scenario
and includes vacuum cleaning of textile once a month. The PCR does not provide detailed guidelines for what should be included in the use stage. In the
end of life stage, the transport distance for waste to waste processing is 72 km (C1). The reuse, recovery and recycling stage is beyond the system boundaries
(D). It is assumed that the solution is dismantled and the materials recycled or combusted according to general Norwegian treatment of industrial waste (see
the table below). This calculation includes only CO2 emissions (GWP) in the C-modules. The transport distance to reuse, recovery or recycling varies for each
material, but the average distance is 373 km. The vehicles used and associated data are described in detail in [5].
Transport from production place to user (A4)
Capacity utilisation Fuel/Energy
Type Type of vehicle Distance km Unit Value (l/t)
(incl. return) % consumption
Truck 38,8 % Truck, 16-32 tonnes, EURO 5 942 0,044606 l/tkm 42,02
Railway l/tkm
Boat l/tkm
Other Transportation l/tkm
NEPD-3253-1894-EN Bo Dining table 180 x 90 cm
5 / 8
LCA: Results
The LCA results are presented below for the declared unit defined on page 2 of the EPD document.
System boundaries (X=included, MND=module not declared, MNR=module not relevant)
Construction Beyond the
Product stage installation User stage End of life stage . system
stage bondaries
A1 A2 A3 A4 A5 B1 B2 B3 B4 B5 B6 B7 C1 C2 C3 C4 . D
X X X X MND MND MND MND MND MND MND MND MND MND MND MND . MND
Environmental impact
Parameter Unit A1 A2 A3 A4
GWP kg CO 2 -eq 3,35E+01 9,74E-01 1,09E+01 6,72E+00
ODP kg CFC11 -eq 2,60E-06 1,79E-07 5,19E-07 1,24E-06
POCP kg C 2H 4-eq 1,85E-02 1,60E-04 2,04E-03 1,09E-03
AP kg SO 2 -eq 1,75E-01 3,24E-03 5,03E-02 2,14E-02
EP kg PO 3- -eq 3,71E-02 5,95E-04 6,69E-03 3,55E-03
4
ADPM kg Sb -eq 2,84E-04 3,19E-06 1,62E-05 2,05E-05
ADPE MJ 3,91E+02 1,46E+01 1,16E+02 1,01E+02
GWP Global warming potential; ODP Depletion potential of the stratospheric ozone layer; POCP Formation potential of tropospheric photochemical oxidants;
AP Acidification potential of land and water; EP Eutrophication potential; ADPM Abiotic depletion potential for non fossil resources; ADPE Abiotic depletion
potential for fossil resources
Reading example: 9,0 E-03 = 9,0*10-3 = 0,009
*INA Indicator Not Assessed
waR slairetam tropsnarT gnirutcafunaM tropsnarT ylbmessA esU ecnanetniaM riapeR tnemecalpeR tnemhsibrufeR lanoitarepO ygrene esu lanoitarepO esu
retaw
-eD noitcurtsnoc noitilomed tropsnarT etsaW gnissecorp lasopsiD -yrevoceR-esueR -gnilcyceR laitnetop
NEPD-3253-1894-EN Bo Dining table 180 x 90 cm
6 / 8
Resource use
Parameter Unit A1 A2 A3 A4
RPEE MJ 1,09E+03 2,15E-01 1,84E+01 1,48E+00
RPEM MJ 8,58E+02 0,00E+00 0,00E+00 0,00E+00
TPE MJ 1,95E+03 2,15E-01 1,84E+01 1,48E+00
NRPE MJ 4,37E+02 1,50E+01 2,03E+02 1,04E+02
NRPM MJ 1,21E+01 0,00E+00 0,00E+00 0,00E+00
TRPE MJ 4,49E+02 1,50E+01 2,03E+02 1,04E+02
SM kg 4,43E+00 0,00E+00 0,00E+00 0,00E+00
RSF MJ 0,00E+00 0,00E+00 0,00E+00 0,00E+00
NRSF MJ 0,00E+00 0,00E+00 0,00E+00 0,00E+00
W m3 3,33E-01 2,80E-03 1,04E-01 1,94E-02
RPEE Renewable primary energy resources used as energy carrier; RPEM Renewable primary energy resources used as raw materials; TPE Total use of renewable
primary energy resources; NRPE Non renewable primary energy resources used as energy carrier; NRPM Non renewable primary energy resources used as
materials; TRPE Total use of non renewable primary energy resources; SM Use of secondary materials; RSF Use of renewable secondary fuels; NRSF Use of non
renewable secondary fuels; W Use of net fresh water
Reading example: 9,0 E-03 = 9,0*10-3 = 0,009
*INA Indicator Not Assessed
End of life - Waste
Parameter Unit A1 A2 A3 A4
HW kg 2,68E-03 9,03E-06 3,08E-02 6,05E-05
NHW kg 2,77E+01 7,64E-01 2,77E+00 5,45E+00
RW kg INA* INA* INA* INA*
HW Hazardous waste disposed; NHW Non hazardous waste disposed; RW Radioactive waste disposed
Reading example: 9,0 E-03 = 9,0*10-3 = 0,009
*INA Indicator Not Assessed
End of life - Output flow
Parameter Unit A1 A2 A3 A4
CR kg 0,00E+00 0,00E+00 0,00E+00 0,00E+00
MR kg 0,00E+00 0,00E+00 4,88E-01 0,00E+00
MER kg 0,00E+00 0,00E+00 0,00E+00 0,00E+00
EEE MJ INA* INA* INA* INA*
ETE MJ INA* INA* INA* INA*
CR Components for reuse; MR Materials for recycling; MER Materials for energy recovery; EEE Exported electric energy; ETE Exported thermal energy
Reading example: 9,0 E-03 = 9,0*10-3 = 0,009
*INA Indicator Not Assessed
NEPD-3253-1894-EN Bo Dining table 180 x 90 cm
7 / 8
Additional Norwegian requirements
Greenhouse gas emissions from the use of electricity in the manufacturing phase
National production mix from import, low voltage (production of transmission lines, in addition to direct emissions and losses in grid) of applied electricity for the manufacturing
process (A3).
Electricity mix Data source Amount Unit
Energy, electricity, European average: 1 kWh ecoinvent 3.4 594,20 g CO2-ekv/kWh
Dangerous substances
The product contains no substances given by the REACH Candidate list or the Norwegian priority list.
Indoor environment
Our Furniture not contain any substances that affects indoor climate.
Additional environmental information
Key environmental indicators for variants for this EPD: Cradle to Gate analyse from A1 to A3
Global warming (kg Share of recycled
Variant number Total energy use (MJ)
CO2) material in product(%)
Bo Dining table 140 x 90 cm 39,80 1 513,47 9,62
Bibliography
ISO 14025:2010 Environmental labels and declarations - Type III environmental declarations - Principles and procedures.
ISO 14044:2006 Environmental management - Life cycle assessment - Requirements and guidelines.
EN 15804:2012+A1:2013 Environmental product declaration - Core rules for the product category of construction products.
ISO 21930:2017 Sustainability in buildings and civil engineering works - Core rules for environmental product declarations of construction products.
ecoinvent v3, Allocation, cut-off by classification, Swiss Centre of Life Cycle Inventories.
Iversen et al., (2018) eEPD v3.0 - Background information for EPD generator system. LCA.no report number 04.18
Vold et al., (2019) EPD generator for Norsk Industri, Background information for industry application and LCA data, LCA.no report number 06.19.
NPCR Part A: Construction products and services. Ver. 1.0. April 2017, EPD-Norge.
NPCR 026 Part B for Furniture. Ver. 2.0 October 2018, EPD-Norge.
Program operator and publisher Phone: +47 23 08 80 00
The Norwegian EPD Foundation e-mail: post@epd-norge.no
Post Box 5250 Majorstuen, 0303 Oslo,Norway web: www.epd-norge.no
Owner of the declaration Phone: +47 958 09 013
Helland Møbler AS e-mail: joakim.helland@helland.no
Postboks 10 6259 Stordal web: www.helland.no
Author of the Life Cycle Assessment Phone: +47 916 50 916
LCA.no AS e-mail: post@lca.no
Dokka 1C 1671 Kråkerøy web: www.lca.no
Developer of EPD generator Phone: +47 916 50 916
LCA.no AS e-mail: post@lca.no
Dokka 1C 1671 Kråkerøy web: www.lca.no
NEPD-3253-1894-EN Bo Dining table 180 x 90 cm
8 / 8
