ENVIRONMENTAL PRODUCT DECLARATION
as per ISO 14025 and EN 15804+A2
Owner of the Declaration dormakaba International Holding GmbH
Publisher Institut Bauen und Umwelt e.V. (IBU)
Programme holder Institut Bauen und Umwelt e.V. (IBU)
Declaration number EPD-DOR-20220165-CBA1-EN
Issue date 30/06/2023
Valid to 29/06/2028
Floor spring BTS 65
dormakaba
www.ibu-epd.com | https://epd-online.com
General Information
dormakaba Floor spring BTS 65
Programme holder Owner of the declaration
IBU – Institut Bauen und Umwelt e.V. dormakaba International Holding GmbH
Hegelplatz 1 DORMA Platz 1
10117 Berlin 58256 Ennepetal
Germany Germany
Declaration number Declared product / declared unit
EPD-DOR-20220165-CBA1-EN 1 piece of the product: Floor spring BTS 65, consisting of the following
items:
• Floor spring
• Product packaging
This declaration is based on the product category rules: Scope:
Building Hardware products, 01/08/2021 This Environmental Product Declaration refers to a specific floor spring
(PCR checked and approved by the SVR) manufactured by dormakaba. The production site is located in Suzhou
(China).
The data represents the year 2020.
Issue date The owner of the declaration shall be liable for the underlying information
and evidence; the IBU shall not be liable with respect to manufacturer
30/06/2023
information, life cycle assessment data and evidences.
The EPD was created according to the specifications of EN 15804+A2. In
Valid to
the following, the standard will be simplified as EN 15804.
29/06/2028
Verification
The standard EN 15804 serves as the core PCR
Independent verification of the declaration and data according to ISO
14025:2011
internally X externally
Dipl.-Ing. Hans Peters
(Chairman of Institut Bauen und Umwelt e.V.)
Florian Pronold Dr.-Ing. Wolfram Trinius,
(Managing Director Institut Bauen und Umwelt e.V.) (Independent verifier)
1 Environmental Product Declaration - dormakaba - Floor spring BTS 65
Product
Performance data of the product with respect to its
Product description/Product definition characteristics in accordance with the relevant technical
The economic floor spring specially designed for double action provision which can be applied are mentioned above.
doors. The BTS 65 offers a particularly shallow design and thus
all the advantages of a reduced installation depth. With two Base materials/Ancillary materials
closing ranges and a choice of models, the BTS 65 can fulfil Name Value Unit
virtually any application requirement while providing all the
Steel 89 %
reliability associated with assured quality.
Zinc 5 %
Lubricant 3 %
For the use and application of the product the respective
national provisions at the place of use apply. The standards Paper 2 %
which can be applied are the following: Aluminium 1 %
• EN 1154 The product includes partial articles which contain substances
• EN 1634-1 listed in the Candidate List of REACH Regulation
1907/2006/EC (date: 17.01.2022) exceeding 0.1 percentage by
Application
mass: yes
The practical clamp fixing system of the BTS 65 ensures a
• Lead (Pb): 7439-92-1 (CAS-No.) is included in some of
secure and high-precision fit in the cement box for double
the alloys used. The concentration of lead in each
action doors, with hydraulic fully controlled closing from approx.
individual alloy does not exceed 4.0% (by mass).
130°.
The Candidate List can be found on the ECHA website
Technical Data address: https:echa.europa.eu/de/home.
The door closers have following technical properties:
Reference service life
The reference service life of the BTS 65 floor spring amounts to
20 years and depends on the application and frequency of use.
For repairs or renewals, suitable spare parts are available. The
floor springs are certified to EN 1154, meaning they are
designed to withstand a minimum of 500.000 cycles.
LCA: Calculation rules
Declared Unit System boundary
The declared unit is 1 piece of the product including the The type of EPD is: cradle to gate with options,
packaging: BTS 65. modules C1–C4, and module D
Name Value Unit (A1–A3 + C + D and additional modules: A4 + A5)
Declared unit 1 piece/product
Production - Module A1-A3
Mass of declared Product 4.1 kg
The product stage includes:
For IBU core EPDs (where clause 3.6 is part of the EPD): for — A1, raw material extraction, processing and
average EPDs, an estimate of the robustness of the LCA mechanical treatments, processing of secondary
values must be made, e.g. concerning the variability of the material input (e.g. recycling processes),
production process, geographical representativeness and the — A2, transport to the manufacturer,
influence of background data and preliminary products — A3, manufacturing and assembly
compared to the environmental impacts caused by the actual including provision of all materials, products and energy, as well
production. as waste processing up to the end-of waste state.
2 Environmental Product Declaration - dormakaba - Floor spring BTS 65
Module D (Benefits and loads beyond the system
Construction stage - Modules A4-A5 boundary) includes:
The construction process stage includes: — D, recycling potentials, expressed as net impacts
— A4, transport to the building site; and benefits.
— A5, installation into the building;
including provision of all materials, products and energy, as well Geographic Representativeness
as waste processing up to the end-of waste state or disposal of Land or region, in which the declared product system is
final residues during the construction process stage. manufactured, used or handled at the end of the product´s
lifespan: China
End-of-life stage– Modules C1-C4 and D
The end-of-life stage includes:
Comparability
— C1, de-construction, demolition:
Basically, a comparison or an evaluation of EPD data is only
— C2, transport to waste processing;
possible if all the data sets to be compared were created
— C3, waste processing for reuse, recovery and/or
according to EN 15804 and the building context, respectively
recycling;
the product-specific characteristics of performance, are taken
— C4, disposal;
into account.
including provision and all transport, provision of all
materials, products and related energy and water use.
LCA: Scenarios and additional technical information
scaling to a specific point of installation, 100 km are declared.
Characteristic product properties of biogenic carbon
The biogenic carbon content quantifies the amount of biogenic
Installation into the building (A5)
carbon in a construction product leaving the factory gate, and it
shall be separately declared for the product and for any Name ValueUnit
accompanying packaging. Output substances following waste treatment on
0.075 kg
If the total mass of biogenic carbon containing materials is less site (packaging)
than 5 % of the total mass of the product and accompanying
packaging, the declaration of biogenic carbon content may be
omitted. The mass of packaging containing biogenic carbon End of life (C1-C4)
shall always be declared. C1: The product dismantling from the building is done manually
without environmental burden.
Note: 1 kg of biogenic carbon is equivalent to 44/12 kg of CO2. C2: Transport to waste treatment at end of life is 50 km.
Name Value Unit
Information on describing the biogenic Carbon Content at Collected separately waste type waste type 4.02 kg
factory gate Recycling 3.89 kg
Name ValueUnit Energy recovery 0.005 kg
Biogenic carbon content in accompanying kg Final disposal 0,13 kg
0.03
packaging C
The product is disassembled in a recycling process. Material
recycling is then assumed for the metals. The plastic
components are assumed to be incinerated with energy
recovery. Minor proportions of residues arising from the
Transport to the building site (A4) recycling process are landfilled. Region for the End of Life is:
Global.
Name Value Unit
Litres of fuel truck (per piece) 0.00276l/100km
Reuse, recovery and/or recycling potentials (D), relevant
Transport distance via truck (for scaling) 100 km
scenario information
Capacity utilisation (including empty runs)
55 % Name Value Unit
average
Recycling 100 %
Transport distance via ship 10000 km
Collection rate is 100%.
The product is transported via truck and ship. The main
distribution regions are China, UAE and India. In order to allow
3 Environmental Product Declaration - dormakaba - Floor spring BTS 65
LCA: Results
DESCRIPTION OF THE SYSTEM BOUNDARY (X = INCLUDED IN LCA; ND = MODULE OR INDICATOR NOT DECLARED; MNR =
MODULE NOT RELEVANT)
Benefits and
Construction loads beyond
Product stage Use stage End-of-life stage
process stage the system
boundaries
la ire ta m w a Ry lp p u s tro p s n a rT g n iru tc a fu n a M e h t m o rf tro p s n a rTe tis e h t o t e ta g y lb m e s s A e s U e c n a n e tn ia M ria p e R tn e m e c a lp e R tn e m h s ib ru fe R y g re n e la n o ita re p Oe s u re ta w la n o ita re p Oe s u n o itc u rts n o c -e Dn o itilo m e d tro p s n a rT g n is s e c o rp e ts a W la s o p s iD -e s u e R-y re v o c e R-g n ilc y c e Rla itn e to p
A1 A2 A3 A4 A5 B1 B2 B3 B4 B5 B6 B7 C1 C2 C3 C4 D
X X X X X MND MND MNR MNR MNR MND MND X X X X X
RESULTS OF THE LCA - ENVIRONMENTAL IMPACT according to EN 15804+A2: 1 door closer
Parameter Unit A1-A3 A4 A5 C1 C2 C3 C4 D
GWP-total kg CO 2 eq 1.18E+01 1.7E-01 1.06E-01 0 1.76E-02 1.19E-02 1.98E-03 -4.01E+00
GWP-fossil kg CO 2 eq 1.19E+01 1.68E-01 2.66E-03 0 1.68E-02 1.19E-02 1.97E-03 -4.01E+00
GWP-biogenic kg CO 2 eq -9.65E-02 1.76E-03 1.04E-01 0 7.76E-04 2.78E-07 6.72E-06 -7.03E-03
GWP-luluc kg CO 2 eq 8.16E-03 3.58E-06 1.75E-06 0 4E-07 6.75E-07 5.66E-06 -3.72E-04
ODP kg CFC11 eq 1.02E-12 1.63E-17 1.92E-17 0 1.77E-18 6.02E-18 7.29E-18 -1.08E-12
AP mol H+ eq 3.58E-02 4.97E-03 2.98E-05 0 1.68E-05 2.13E-06 1.41E-05 -1.09E-02
EP-freshwater kg P eq 1.79E-05 3.75E-08 3.75E-09 0 3.59E-09 9.61E-10 3.38E-09 -3.94E-06
EP-marine kg N eq 7.31E-03 1.31E-03 1.08E-05 0 5.35E-06 4.8E-07 3.63E-06 -1.81E-03
EP-terrestrial mol N eq 7.88E-02 1.44E-02 1.34E-04 0 5.94E-05 9.69E-06 3.99E-05 -1.86E-02
kg NMVOC
POCP 2.29E-02 3.67E-03 2.85E-05 0 1.51E-05 1.33E-06 1.1E-05 -7.18E-03
eq
ADPE kg Sb eq 1E-03 4.47E-09 3.03E-10 0 5.03E-10 8.26E-11 1.77E-10 -3.46E-04
ADPF MJ 1.34E+02 2.11E+00 3.36E-02 0 2.38E-01 5.54E-03 2.58E-02 -3.84E+01
m3 world eq
WDP 1.66E+00 3.08E-04 1.32E-02 0 3.29E-05 1.22E-03 2.06E-04 -3.89E-01
deprived
GWP = Global warming potential; ODP = Depletion potential of the stratospheric ozone layer; AP = Acidification potential of land and water; EP =
Eutrophication potential; POCP = Formation potential of tropospheric ozone photochemical oxidants; ADPE = Abiotic depletion potential for non-fossil
resources; ADPF = Abiotic depletion potential for fossil resources; WDP = Water (user) deprivation potential)
RESULTS OF THE LCA - INDICATORS TO DESCRIBE RESOURCE USE according to EN 15804+A2: 1 door closer
Parameter Unit A1-A3 A4 A5 C1 C2 C3 C4 D
PERE MJ 2.54E+01 6.85E-03 9.06E-01 0 7.51E-04 1.41E-01 3.38E-03 -7.97E-01
PERM MJ 1.04E+00 0 -9E-01 0 0 -1.39E-01 0 0
PERT MJ 2.65E+01 6.85E-03 6.1E-03 0 7.51E-04 1.44E-03 3.38E-03 -7.97E-01
PENRE MJ 1.34E+02 2.11E+00 3.36E-02 0 2.38E-01 1.25E-01 2.58E-02 -3.84E+01
PENRM MJ 1.19E-01 0 0 0 0 -1.19E-01 0 0
PENRT MJ 1.35E+02 2.11E+00 3.36E-02 0 2.38E-01 5.54E-03 2.58E-02 -3.84E+01
SM kg 2.04E+00 0 0 0 0 0 0 0
RSF MJ 0 0 0 0 0 0 0 0
NRSF MJ 0 0 0 0 0 0 0 0
FW m3 5.48E-02 1.24E-05 3.1E-04 0 1.35E-06 2.92E-05 6.51E-06 -1.19E-02
PERE = Use of renewable primary energy excluding renewable primary energy resources used as raw materials; PERM = Use of renewable primary
energy resources used as raw materials; PERT = Total use of renewable primary energy resources; PENRE = Use of non-renewable primary energy
excluding non-renewable primary energy resources used as raw materials; PENRM = Use of non-renewable primary energy resources used as raw
materials; PENRT = Total use of non-renewable primary energy resources; SM = Use of secondary material; RSF = Use of renewable secondary fuels;
NRSF = Use of non-renewable secondary fuels; FW = Use of net fresh water
RESULTS OF THE LCA – WASTE CATEGORIES AND OUTPUT FLOWS according to EN 15804+A2:
1 door closer
Parameter Unit A1-A3 A4 A5 C1 C2 C3 C4 D
HWD kg 1.5E-07 2.07E-10 4.95E-11 0 2.31E-11 2.11E-11 3.93E-10 -3.77E-06
NHWD kg 3.18E-01 2.16E-04 3.33E-03 0 2.44E-05 1.24E-03 1.3E-01 3.13E-01
RWD kg 4.67E-03 2.33E-06 1.76E-06 0 2.56E-07 2.06E-07 2.94E-07 -7.21E-04
CRU kg 0 0 0 0 0 0 0 0
MFR kg 0 0 0 0 0 3.88E+00 0 0
MER kg 0 0 0 0 0 0 0 0
EEE MJ 0 0 1.61E-01 0 0 0 0 0
EET MJ 0 0 2.92E-01 0 0 0 0 0
4 Environmental Product Declaration - dormakaba - Floor spring BTS 65
HWD = Hazardous waste disposed; NHWD = Non-hazardous waste disposed; RWD = Radioactive waste disposed; CRU = Components for re-use;
MFR = Materials for recycling; MER = Materials for energy recovery; EEE = Exported electrical energy; EET = Exported thermal energy
RESULTS OF THE LCA – additional impact categories according to EN 15804+A2-optional:
1 door closer
Parameter Unit A1-A3 A4 A5 C1 C2 C3 C4 D
Disease
PM 5.09E-07 8.45E-08 1.65E-10 0 8.83E-11 2.71E-11 1.75E-10 -1.57E-07
incidence
IR kBq U235 eq 5.59E-01 3.35E-04 2.73E-04 0 3.65E-05 1.85E-05 3.02E-05 -4.34E-02
ETP-fw CTUe 4.54E+01 1.49E+00 1.59E-02 0 1.69E-01 2.08E-03 1.47E-02 -4.94E+00
HTP-c CTUh 9.1E-09 2.81E-11 8.43E-13 0 3.17E-12 1.8E-13 2.18E-12 3.76E-09
HTP-nc CTUh 2.22E-07 1.3E-09 3.65E-11 0 1.36E-10 1.82E-11 2.41E-10 2.94E-07
SQP SQP 3.47E+01 5.56E-03 8.9E-03 0 6.12E-04 1.66E-03 5.38E-03 1.54E-01
PM = Potential incidence of disease due to PM emissions; IR = Potential Human exposure efficiency relative to U235; ETP-fw = Potential comparative
Toxic Unit for ecosystems; HTP-c = Potential comparative Toxic Unit for humans (cancerogenic); HTP-nc = Potential comparative Toxic Unit for humans
(not cancerogenic); SQP = Potential soil quality index
Disclaimer 1 – for the indicator “Potential Human exposure efficiency relative to U235”. This impact category deals mainly with the
eventual impact of low-dose ionizing radiation on human health of the nuclear fuel cycle. It does not consider effects due to possible
nuclear accidents, occupational exposure or radioactive waste disposal in underground facilities. Potential ionizing radiation from the
soil, radon and from some construction materials is also not measured by this indicator.
Disclaimer 2 – for the indicators “abiotic depletion potential for non-fossil resources”, “abiotic depletion potential for fossil resources”,
“water (user) deprivation potential, deprivation-weighted water consumption”, “potential comparative toxic unit for ecosystems”,
“potential comparative toxic unit for humans – cancerogenic”, “Potential comparative toxic unit for humans - not cancerogenic”,
“potential soil quality index”. The results of this environmental impact indicator shall be used with care as the uncertainties on these
results are high as there is limited experience with the indicator.
This EPD was created using a software tool.
References
e.V., 2021. www.ibu-epd.com
EN 1154
EN 1154-2003; GaBi
Building hardware - Controlled door closing devices - Sphera Solutions GmbH
Requirements and test methods Gabi Software System and Database for Life Cycle Engineering
1992-2020
EN 1634-1 Version 10.0.0.71
EN 1634-1:2018; Fire resistance and smoke control tests for University of Stuttgart
door and shutter assemblies, Leinfelden-Echterdingen
openable windows and elements of building hardware - Part 1:
Fire GaBi ts documentation
resistance test for door and shutter assemblies and openable GaBi life cycle
windows inventory data documentation
(https://www.gabi-software.com/support/gabi/gabidatabase-
EN 15804+A2 2020-lci-documentation/)
EN 15804:2019+A2 (in press), Sustainability of construction
works — Environmental Product LCA-tool dormakaba
Declarations — Core rules for the product category of LCA-tool, IBU-DOR-202104-LT1-EN, 2021,
construction products developed by Sphera Solutions GmbH
REACH Regulation 1907/2006/EC PCR Part A
Regulation (EC) No 1907/2006 of the European Parliament and PCR – Part A: Calculation Rules for the Life Cycle Assessment
of the Council on the Registration, Evaluation, Authorisation and Requirements on the Project Report according to EN
and Restriction of Chemicals (REACH) 15804+A2:2019, Version 1.0, 2020, Institut Bauen und Umwelt
e.V., www.ibu-epd.com
Further References
PCR Part B
IBU 2021 PCR – Part B: Requirements on the EPD for Building Hardware
General Instructions for the EPD programme of Institut Bauen product, version 1.2, Institut Bauen und Umwelt e.V., www.ibu-
und Umwelt e.V. Version 2.0, Berlin: Institut Bauen und Umwelt epd.com, 2017
5 Environmental Product Declaration - dormakaba - Floor spring BTS 65
Publisher
Institut Bauen und Umwelt e.V. +49 (0)30 3087748- 0
Hegelplatz 1 info@ibu-epd.com
10117 Berlin www.ibu-epd.com
Germany
Programme holder
Institut Bauen und Umwelt e.V. +49 (0)30 3087748- 0
Hegelplatz 1 info@ibu-epd.com
10117 Berlin www.ibu-epd.com
Germany
Author of the Life Cycle Assessment
dormakaba International Holding GmbH +49 2333 793-0
DORMA Platz 1 info.de@dormakaba.com
58256 Ennepetal www.dormakaba.com
Germany
Owner of the Declaration
dormakaba International Holding GmbH +49 2333 793-0
DORMA Platz 1 info.de@dormakaba.com
58256 Ennepetal www.dormakaba.com
Germany
6 Environmental Product Declaration - dormakaba - Floor spring BTS 65
