ENVIRONMENTAL PRODUCT DECLARATION
as per ISO 14025 and EN 15804+A1
Owner of the Declaration NMC S.A.
Programme holder Institut Bauen und Umwelt e.V. (IBU)
Publisher Institut Bauen und Umwelt e.V. (IBU)
Declaration number EPD-NMC-20210311-IBD1-EN
Issue date 05.01.2022
Valid to 04.01.2027
CLIMAFLEX®naturefoam stabil
NMC S.A.
www.ibu-epd.com | https://epd-online.com
Umwelt Produktdeklaration Name des Herstellers – Name des Produkts
1. General Information
NMC S.A. CLIMAFLEX®naturefoam stabil
Programme holder Owner of the declaration
IBU – Institut Bauen und Umwelt e.V. NMC S.A.
Panoramastr. 1 Gert-Noel Strasse
10178 Berlin BE-4731 Eynatten
Germany
Declaration number Declared product / declared unit
EPD-NMC-20210311-IBD1-EN 1 m³ insulation material CLIMAFLEX®naturefoam
stabil
This declaration is based on the product Scope:
category rules: Product line CLIMAFLEX®naturefoam stabil
Insulating materials made of foam plastics, 01.2019 Thermal insulation products for building equipment and
(PCR checked and approved by the SVR) industrial insulations made of Polythene-based, closed-
cell foam pipe insulation with a robust protective
Issue date coating (PEF) according to /EN14313/. This declaration
is an Environmental Product Declaration according to
05.01.2022
/ISO14025/ describing the specific environmental
performance of the product produced in Belgium at the
Valid to
site of Eynatten.
04.01.2027
The owner of the declaration shall be liable for the
underlying information and evidence; the IBU shall not
be liable with respect to manufacturer information, life
cycle assessment data and evidences.
The EPD was created according to the specifications
of EN 15804+A1. In the following, the standard will be
simplified as EN 15804.
Verification
The standard EN 15804 serves as the core PCR
Independent verification of the declaration and data
according to ISO 14025:2010
Dipl. Ing. Hans Peters internally x externally
(chairman of Institut Bauen und Umwelt e.V.)
Dr. Alexander Röder Vito D'Incognito
(Managing Director Institut Bauen und Umwelt e.V.)) (Independent verifier)
2. Product
2.1 Product description/Product definition  Products made of PE foam yield an excellent
CLIMAFLEX®naturefoam stabil is the Professional cost/performance ratio.
Polythene-based closed-cell foam pipe insulation with
 Heat loss control and noise reduction in fresh-
a robust PE protective coating for continues energy
and waste water and heating systems
saving and condensation control purposes.
CLIMAFLEX®naturefoam stabil provides solutions that
follow all necessary guidelines for any type of
installation. 2.3 Technical Data
For the placing on the market of the product in the
European Union/European Free Trade Association
(EU/EFTA) (with the exception of Switzerland) - Constructional data
Thermal Insulation products for building equipment and Name Value Unit
industrial installations. Factory made polyethylene Gross density 26.5 kg/m3
foam (PEF) and the CE-marking. For the application Thermal conductivity λ at 40°C 0.04 W/(mK)
and use, the respective national provisions apply. Reaction to fire acc.to /EN 13501-
E -
1/
2.2 Application Max Service Temperature acc. To
100 °C
CLIMAFLEX®naturefoam stabil is used to insulate /EN14706/, /EN 14707
pipes for heating and plumbing. Min Service Temperature 0 °C
 Polyethylene foam is a cost-efficient material Water absorption acc. to /EN
WS005
with good insulating properties. 13472/
2 Environmental Product Declaration NMC sa – CLIMAFLEX®naturefoam stabil
Traces quantities of water soluble Cl < 20 – F flowable thermoplastic mass. The thermoplastic mass
ions and pH-value acc. to EN < 4 - pH is then metered to a mixing zone where the
13468 and EN 13472 5,8 thermoplastic mass is thoroughly mixed with a blowing
agent under pressure. The mixture of thermoplastic
resin and blowing agent is then forced through a die,
which imparts a shape to the thermoplastic mass, into
a zone of lower pressure, such as atmospheric
2.4 Delivery status pressure. The blowing agent expands to form the cells
The PE products are supplied as tubes. The tubes are of the foam and the thermoplastic foam is cooled
delivered in lengths of 2 m packed in cardboard boxes. trough an inline water cooler. The protection coating
The insulating sleeves in the CLIMAFLEX®naturefoam "skin" is applied by co-extrusion. The "skin" is made
stabil have a thickness ranging from 4 to 25 mm and with solid pellets of thermoplastic resin and some
an inside diameter ranging from 15 to 42 mm. These additives, which is, with the help of an extruder,
products are categorized according to thermal applied around the foam. There's no a foaming agent
conductivity (Lambda*). The category of product with used in this case. The die is positioned around the
lambda 0,040 (W/(mK)) (acc. to /EN ISO 8497/ and "naked" foam and deposes a small thickness (± 0.1
/EN 12667/). mm) of PE film on the foam. At the end of this process
the profiles are cut at dimension.
2.5 Base materials/Ancillary materials
Quality assurance :
Base materials The manufacture is certified /ISO 9001/ for the quality
CLIMAFLEX®naturefoam stabil is a flexible insulation management. The product corresponds to the product
material based on Polyethylene with a protecting standard /EN 14313/ and have a Declaration of
coating of PE., which consists of around 7 basic Performance according the /CPR/ : DOP no.
components. The following table displays the different W1PEF300 ; W1PEF400 (see www.nmc-
elements of the formula. insulation.com)
This product contains substances listed in the
candidate list (date: 08.07.2021) exceeding 0.1
percentage by mass: No. 2.7 Environment and health during
This product contains other CMR substances in manufacturing
categories 1A or 1B, which are not on the candidate During all manufacturing steps of NMC S.A. Belgium,
list, exceeding 0.1 percentage by mass: No. the production follows the national guidelines and
Biocide products were added to this construction regulations. Solar panels are installed on the roof of
product or it has been treated with biocide products the warehouses.
(this then concerns a treated product as defined by the
(EU) Ordinance on Biocide Products No. 2.8 Product processing/Installation
528/2012): No. CLIMAFLEX®naturefoam stabil can be installed using
basic tools like knives. No special tools, or specific
protection is necessary. When applying adhesives the
information given in the relevant safety data sheets is
to be heeded. The recommendations on how to use
Name Value Unit the product are described in the application manuals or
BIO LDPE 51,68 % video's. More details are listed on the Web Page
Polyethylene 20,7 % www.nmc-insulation.com
NMC Internally recycled PE 14,94 %
Flame retardant 1,74 % 2.9 Packaging
Pigments and fillers 2,32 % CLIMAFLEX®naturefoam stabil products are packed
Volume stabilizer 0,97 % in cardboard boxes and transported on reusable
Blowing Agent 7,65 % pallets. The packaging material can be recycled. The
PE and fillers give the aspect of the product. The pallets used to transport the products are taken back
blowing agent causes the expansion during or exchanged when the CLIMAFLEX®naturefoam
manufacturing and the flame retardants ensure the fire stabil is delivered, so the use of pallets is a close loop
resistance. According to the European Chemicals economy
Regulation /REACH/ Manufacturers, importers and
downstream users must register their chemicals and
are responsible for their safe use on their own. For its 2.10 Condition of use
production NMC S.A. uses exc lusively verifiably During the use of the product for the purpose for
registered and approved substances. Products which they are intended, there are no modifications on
manufactured and put on the market by NMC need to the product during the use, except if due to
be registered. CLIMAFLEX®naturefoam stabil does extraordinary impact (see point 2.13).
not contain Substances of Very High Concern (SVHC).
Antimony trioxide and halogenated flame retardants 2.11 Environment and health during use
are applied. There are no particular aspects of the material
composition during the use. CLIMAFLEX®naturefoam
stabil products are used in a wide range and varieties
of applications for which the product is intended to.
2.6 Manufacture The PEF foams fulfil the German, Belgian and French
The manufacturing process consists of a continuous regulations regarding the emission of VOC with
extrusion. Solid pellets of thermoplastic resin are fed to emissions far below the most severe limit values. The
a melting zone in which the resin is melted, to form a Eurofin Product Testing institute, on the demand of
the CEFEP (European group of PEF and FEF
3 Environmental Product Declaration NMC sa – CLIMAFLEX®naturefoam stabil
manufacturers) has made a wide range of tests for
different PEF products from different manufacturers. Water
The insulation of heating pipes with CLIMAFLEX®naturefoam stabil are closed cell foam
CLIMAFLEX®naturefoam stabil allows a drastic and obtain the better water absorption class WS005
reduction of CO emission during the full service live of according to the product standard
2
the installation. The quantification of this is not in the
topic of this EPD, and has to be evaluated in the frame Mechanical destruction
of the LCA from the complete installation CLIMAFLEX®naturefoam stabil are flexible foam
covered with a PE protective coating
2.12 Reference service life CLIMAFLEX®naturefoam stabil are not UV resistant.
The function of CLIMAFLEX®naturefoam stabil is to The use is not recommended for outside applications
ensure the insulation of heating and sanitary without complementary UV protection.
installations for a reference service life (RSL) of 50
years. This duration is based on the frequency of 2.14 Re-use phase
replacement of sanitary and heating piping in buildings. In principle, if removed carefully,
Although the insulation products are still effective after CLIMAFLEX®naturefoam stabil can be reused on any
50 years, it is assumed that when replacing the piping, other piping system of similar dimensions. Any material
the insulation is not reused and is disposed of with the not suitable for reuse is fully recyclable.
piping. 50 years is the minimum Reference Service
Life recommended in /EN16783/ . 2.15 Disposal
CLIMAFLEX®naturefoam stabil are fully recyclable
using the same recycling systems as those used for
2.13 Extraordinary effects other forms of PE waste.
Any non-recycled material should be disposed of the
Fire materials according to the local regulations, and by the
According to CLIMAFLEX®naturefoam stabil are European Waste Catalogue waste code 07 02 13
classified as EURO CLASS E and therefore have a waste Plastic "Low Density Polyethylene"
limited speed of inflammation.
2.16 Further information
Additional information about CLIMAFLEX®naturefoam
stabil can be found on the NMC web site www.nmc-
Fire Protection insulation.com. Here specification clauses, data sheets
Name Value and application manuals can be found.
Building material class E
3. LCA: Calculation rules
3.1 Declared Unit to the environmental impacts caused by actual
The declaration refers to 1 m³ of produced insulation production.
product. For the LCA calculations, as the product is
foam and has some tolerances, the density declared is 3.2 System boundary
the average between the product categories. The The Data collection refers to the yearly production in
thermal conductivity coefficient (Lambda-value) and R- 2020.
value per 25 mm thickness per product brand is Module A1 to A3: The LCA calculation covers the
provided below as additional information and support production of the raw materials, transport of these to
for installers. the plant, the mixing of raw materials according to the
respective recipes, manufacturing of the foam product
Name Value Unit and packaging for dispatch. All production takes place
Declared unit 1 m3 exclusively in Eynatten, Belgium.
Gross density 26.5 kg/m3 Module A4: Transport of the final product to the
Volume for 1kg 0,03772 m³ application site. The average transport distance has
Grammage - kg/m2 been calculated based on a weighted value for NMC’s
Value for 1 main customers representing more than 50% of the
m3 sales volume in 2020. Capacity utilisation by volume is
divided 100%. However, given the low density of the product,
Conversion Factor from 1 m3 to 1
section of m capacity utilisation by mass has been estimated as
linear meter
the 10%.
insulation Module A5: The products can be placed end to end
pipe ( m²) and the remaining pieces can be reused on other
Thermal Conductivity λ: 0.040 W/mK at (40°C) pipes. The calculations do not contain any installation
R-value- thickness: 25 mm: +/- 3,5 (m²K)/W waste. Cardboard as a packaging material is assumed
depending on the pipe diameter. to be recycled. As input material cardboard made of
waste paper is considered. Thus, the environmental
For IBU core EPDs (where clause 3.6 is part of the burden for packaging material is considered already in
EPD): for average EPDs, an estimate of the A1-A3. The value of the environmental impact for A5 is
robustness of the LCA values must be made, e.g. declared as “0”.
concerning variability of the production process, Module B1-B7:The foam insulation products do not
geographical representativeness and the influence of require maintenance, replacement or refurbishment
background data and preliminary products compared while in use. The information modules B1 – B7 are not
declared. Although the insulation of the piping
4 Environmental Product Declaration NMC sa – CLIMAFLEX®naturefoam stabil
contributes to a significant reduction of CO2 emissions 3.5 Background data
from the heating or cooling equipment, this is not taken The software system for life cycle engineering GaBi
into account in this LCA. It should, however, be taken 2021 life cycle database used in the GaBi 10 software
into account in the calculation of environmental environment (Service Pack 2021001000) developed by
impacts of the complete heating and cooling systems Thinkstep AG was used to perform this LCA. The GaBi
or of the complete building. LCI database /GaBi 7/ provides the life cycle inventory
Module C1: As for the installation of the product, the data for several of the raw and process materials
disassembly is done manually and does not require obtained from the background system.
any specific equipment. Disassembly is generally
carried out at the same time as the replacement or 3.6 Data quality
removal of sanitary pipes. Consequently, there are no All the foreground data requiring such energy or raw
impacts associated with C1. material coming from production, were verified and
Module C2:Transport at end-of-life stage is modeled cross-checked before being included in the model.
as a Euro Cargo 0-6 mix truck with diesel fuel. The Most of the life cycle inventories for the basic materials
average distance to mechanical recycling is assumed are available in the GaBi 7 database.
to be 100 km. For electrical and thermal energy Belgium specific grid
Module C3:. The legislation is pushing more in this mixes and Belgium specific supply for natural gas were
direction and the overall pressure on plastic recycling considered.
is growing, the scenario with 100 % mechanical
recycling is considered. The environmental burden is 3.7 Period under review
declared in module C3. The production data for the year 2020 were used for
the realisation of this study.
Module C4: The environmental burden for 100%
landfilling is 0 because 100 % mechanical recycling is 3.8 Allocation
considered. There is no co-product or by-product generated during
the production of NMC’s products.
Module D: The end-of-life scenarios for packaging Due to lack of specific data per production line and
material and product do not deliver any benefits for the product, the energy has been allocated per overall
next system. Recycling of cardboard is a closed cycle produced volume of insulation foam.
with the production process. The CLIMAFLEX®
naturefoam stabil foam is fully recyclable and can be Production waste
used as a direct one-for-one substitute for virgin PE-LD Most of the production waste from the process
granulates, with only minor additive additions. There is (machine start, end of production, non-conforming
no chemical difference between bio-based PE-LD and products, etc.) is recycled internally in order to be
fossil fuel derived PE-LD, so using a mix of sources reused in the manufacturing process. These impacts
does not change the recyclability of the product. are accounted for in A1-A3. Smaller amounts are
disposed of on a landfill site.
3.3 Estimates and assumptions Installation and End-of-Life waste
The LCA calculation is conducted using the Gabi ts - Installation of the foam products is done by hand and
database. Not all necessary LCIs are included in the requires no special equipment apart from a knife.
database. Where data were missing or were Installation off-cut is not considered in this calculations.
unavailable or where suppliers were unable to provide Any glue and adhesive tapes used during the
complete information, proxy datasets have been used. installation phase were not included in the LCA.
The environmental burden for the production of
pigments, flame retardants and volume stabilizers are 3.9 Comparability
approximated. Basically, a comparison or an evaluation of EPD data
is only possible if all the data sets to be compared
3.4 Cut-off criteria were created according to EN 15804 and the building
Any glue and adhesive tapes used during the context, respectively the product-specific
installation (A5) have not been included as characteristics of performance, are taken into account.
quantification of these materials is uncertain and their
use by the various installers is too diverse, adhesives
and glues are not required in all/most cases, but may
be used for some applications.
In this study no others cut-off criteria have been
applied and all elementary incoming processes as well
as all energy and water inputs and waste outputs have
been counted.
4. LCA: Scenarios and additional technical information
empty runs)
Gross density of products
26.5 kg/m3
Transport to the building site (A4) transported
Name Value Unit
Litres of fuel 0.153 l/100km Installation into the building (A5)
Transport distance 477 km Name Value Unit
Capacity utilisation (including 10 %
5 Environmental Product Declaration NMC sa – CLIMAFLEX®naturefoam stabil
Use or application of the installed product (B1) see
section 2.12 "Use"
Name Value Unit
Maintenance (B2)
Name Value Unit
Auxiliary - kg
Other energy carriers - MJ
Material loss - kg
Repair (B3)
Name Value Unit
Information on the repair process - -
Information on the inspection process - -
Number/
Repair cycle -
RSL
Water consumption - m3
Auxiliary - kg
Other resources - kg
Electricity consumption - kWh
Other energy carriers - MJ
Material loss - kg
Replacement (B4) / Refurbishment (B5)
Name Value Unit
Number/
Replacement cycle -
RSL
Electricity consumption - kWh
Litres of fuel - l/100km
Replacement of worn parts - kg
Reference service life
Name Value Unit
Reference service life 50 a
Operational energy use (B6) and Operational water
use (B7)
Name Value Unit
Water consumption - m3
Electricity consumption - kWh
Other energy carriers - MJ
Equipment output - kW
End of life (C1-C4)
Name Value Unit
Recycling 26.5 kg
6 Environmental Product Declaration NMC sa – CLIMAFLEX®naturefoam stabil
5. LCA: Results
DESCRIPTION OF THE SYSTEM BOUNDARY (X = INCLUDED IN LCA; MND = MODULE NOT DECLARED;
MNR = MODULE NOT RELEVANT)
BENEFITS AND
CONSTRUCTI LOADS
PRODUCT STAGE ON PROCESS USE STAGE END OF LIFE STAGE BEYOND THE
STAGE SYSTEM
BOUNDARIES
7 Environmental Product Declaration NMC sa – CLIMAFLEX®naturefoam stabil
lairetam
waR
ylppus tropsnarT
gnirutcafunaM
eht
morf
tropsnarT
etis
eht
ot
etag
ylbmessA esU
ecnanetniaM
riapeR
tnemecalpeR tnemhsibrufeR
ygrene
lanoitarepO esu
retaw
lanoitarepO esu
noitcurtsnoc-eD
noitilomed tropsnarT
gnissecorp
etsaW
lasopsiD -esueR -yrevoceR -gnilcyceR laitnetop
A1 A2 A3 A4 A5 B1 B2 B3 B4 B5 B6 B7 C1 C2 C3 C4 D
X X X X X MND MND MNR MNR MNR MND MND MND X X X X
RESULTS OF THE LCA - ENVIRONMENTAL IMPACT according to EN 15804+A1: 1 m³
CLIMAFLEX®naturefoam stabil
Parameter Unit A1-A3 A4 A5 C2 C3 C4 D
GWP [kg CO2-Eq.] 22.87 1.54 0.00 0.21 2.28 0.00 -64.37
ODP [kg CFC11-Eq.] 3.85E-8 4.13E-16 0.00E+0 5.62E-17 2.05E-13 0.00E+0 -8.54E-13
AP [kg SO2-Eq.] 7.36E-1 1.52E-3 0.00E+0 1.80E-4 2.36E-3 0.00E+0 -7.32E-2
EP [kg (PO4)3--Eq.] 6.85E-1 3.17E-4 0.00E+0 3.61E-5 5.72E-4 0.00E+0 -1.15E-2
POCP [kg ethene-Eq.] 1.98E-1 -1.67E-4 0.00E+0 2.34E-5 2.73E-4 0.00E+0 -1.30E-2
ADPE [kg Sb-Eq.] 8.21E-2 1.39E-7 0.00E+0 1.90E-8 1.69E-6 0.00E+0 -1.56E-5
ADPF [MJ] 1487.97 20.70 0.00 2.82 30.26 0.00 -2491.94
GWP = Global warming potential; ODP = Depletion potential of the stratospheric ozone layer; AP = Acidification potential of land and water; EP =
Caption Eutrophication potential; POCP = Formation potential of tropospheric ozone photochemical oxidants; ADPE = Abiotic depletion potential for non-
fossil resources; ADPF = Abiotic depletion potential for fossil resources
RESULTS OF THE LCA - INDICATORS TO DESCRIBE RESOURCE USE according to EN 15804+A1: 1 m³
CLIMAFLEX®naturefoam stabil
Parameter Unit A1-A3 A4 A5 C2 C3 C4 D
PERE [MJ] 1685.96 1.20 0.00 0.16 30.63 0.00 -156.75
PERM [MJ] 908.01 0.00 0.00 0.00 0.00 0.00 0.00
PERT [MJ] 2593.97 1.20 0.00 0.16 30.63 0.00 -156.75
PENRE [MJ] 1403.55 20.99 0.00 2.86 91.68 0.00 -2543.94
PENRM [MJ] 394.29 0.00 0.00 0.00 0.00 0.00 0.00
PENRT [MJ] 1797.84 20.99 0.00 2.86 91.68 0.00 -2543.94
SM [kg] 14.32 0.00 0.00 0.00 0.00 0.00 0.00
RSF [MJ] 0.00 0.00 0.00 0.00 0.00 0.00 0.00
NRSF [MJ] 0.00 0.00 0.00 0.00 0.00 0.00 0.00
FW [m³] 0.22 0.00 0.00 0.00 0.02 0.00 -0.29
PERE = Use of renewable primary energy excluding renewable primary energy resources used as raw materials; PERM = Use of
renewable primary energy resources used as raw materials; PERT = Total use of renewable primary energy resources; PENRE = Use of
non-renewable primary energy excluding non-renewable primary energy resources used as raw materials; PENRM = Use of non-
Caption
renewable primary energy resources used as raw materials; PENRT = Total use of non-renewable primary energy resources; SM = Use
of secondary material; RSF = Use of renewable secondary fuels; NRSF = Use of non-renewable secondary fuels; FW = Use of net fresh
water
RESULTS OF THE LCA – WASTE CATEGORIES AND OUTPUT FLOWS according to EN 15804+A1:
1 m³ CLIMAFLEX®naturefoam stabil
Parameter Unit A1-A3 A4 A5 C2 C3 C4 D
HWD [kg] 3.68E-4 1.11E-9 0.00E+0 1.51E-10 3.14E-8 0.00E+0 -2.33E-7
NHWD [kg] 8.24E+0 3.29E-3 0.00E+0 4.48E-4 1.00E-1 0.00E+0 -4.33E-1
RWD [kg] 9.71E-2 3.81E-5 0.00E+0 5.18E-6 2.42E-2 0.00E+0 -1.22E-2
CRU [kg] 0.00 0.00 0.00 0.00 0.00 0.00 0.00
MFR [kg] 0.00 0.00 14.32 0.00 35.30 0.00 0.00
MER [kg] 0.00 0.00 0.00 0.00 0.00 0.00 0.00
EEE [MJ] 0.00 0.00 0.00 0.00 0.00 0.00 0.00
EET [MJ] 0.00 0.00 0.00 0.00 0.00 0.00 0.00
HWD = Hazardous waste disposed; NHWD = Non-hazardous waste disposed; RWD = Radioactive waste disposed; CRU = Components
Caption for re-use; MFR = Materials for recycling; MER = Materials for energy recovery; EEE = Exported electrical energy; EET = Exported
thermal energy
6. LCA: Interpretation
The base polymer used at NMC is produced from A more in-depth analysis of the production module A1
renewable raw materials (Biomass/Sugar cane). One to A3 shows that the production of raw materials and
of the advantages of using a biopolymer is a significant their transport account for most of 85% of the impact
reduction in greenhouse gas emissions compared to Global Warming Potential.
the use of raw materials of fossil origin. In addition, the One way to continue to reduce the environmental
use of non-renewable raw materials is avoided in this impact of the CLIMAFLEX®naturefoam stabil would be
way. to continue to diversify our energy sources by
When we analyse the complete life cycle we see that switching more and more to renewable energies. To
the most impacting part for all environmental impact this end, after having greatly increased the number of
factors is the production module and more particularly photovoltaic panels, NMC will acquire a cogeneration
the raw materials. With regard to global warming for system. One way to continue to reduce the
the complete life cycle, more than 88% comes from the environmental impact of the CLIMAFLEX® naturefoam
production module 1,3 % of transport to the places of stabil would be to continue to diversify our energy
installation and less than 10% comes from the end of sources by switching more and more to renewable
life. For all other impact factors, more than 90% of the energies. To this end, after having greatly increased
impacts come from the production phase. the number of photovoltaic panels, NMC will acquire a
Transport has a more pronounced impact on global cogeneration system. Looking for more eco-
warming potential as well as on soil and water responsible suppliers must also be put in place, as well
acidification potential and abiotic fossil resource as finding raw materials manufactured locally to avoid
depletion potential. long-distance transport as much as possible.
7. Requisite evidence
7.1. VOC emissions VOC Emissions
Eurofins Product Testing A/S has tested a wide range Name Value Unit
and variety of typical PEF (Polyethylene foam) Overview of Results (28 Tage) - μg/m3
products marketed in the EU from CEFEP (European TVOC (C6 - C16) - μg/m3
Group of PEF/FEF manufacturers) Based on the Sum SVOC (C16 - C22) - μg/m3
loading factor 0.05m²/m3 (determined after R (dimensionless) - -
consideration of the real life applications of PEF VOC without NIK - μg/m3
products (in living rooms) and recommendations by the Carcinogenic Substances - μg/m3
experts of the test institute) all results were found to be
clearly below the limit values. For all samples below AgBB overview of results (3 days [µg/m³])
100mg/m3 TVOC after 28 days. Certificates are
Name Value Unit
available on request. TVOC (C6 - C16) - μg/m3
Sum SVOC (C16 - C22) - μg/m3
7.2 Leaching
R (dimensionless) - -
According to /EN 13468/ the content of water-soluble
VOC without NIK - μg/m3
chloride ions for CLIMAFLEX® naturefoam stabil is
Carcinogenic Substances - μg/m3
<20mg/kg.
8. References
EN 1602 ISO 14001
EN 1602: 2013: Thermal insulating products for ISO 14001: 2015 Environmental management
building applications - Determination of the apparent systems.
density
EN ISO 14025
EN ISO 8497 EN ISO 14025: 2011-10: Environmental labels and
EN ISO 8497: Thermal insulation - Determination of declarations — Type III environmental declarations —
steady-state thermal transmission properties of thermal Principles and procedures
insulation for circular pipes
ISO 14040
ISO 9001 ISO 14040: Environmental management — Life cycle
ISO 9001: 2015: Quality management systems. assessment — Principles and framework
EN 13501-1 ISO 14044
EN 13501-1:2007+A1: 2013 Fire classification of ISO 14044: Environmental management — Life cycle
construction products and building elements - assessment — Requirements and guidelines
Classification using test data from reaction to fire tests
EN 14707
8 Environmental Product Declaration NMC sa – CLIMAFLEX®naturefoam stabil
EN 14707: 2012: Thermal insulating products for Eurofins: Product Testing Institute
building equipment and industrial installations.
Determination of maximum service temperature for Gabi ts
preformed pipe insulation GaBi 10 GaBi Software-System and Database for Life
Cycle Engineering Copyright © 1992-2021 Sphera
EN 15804 Solutions Gmbh Version: 10.5.0.78 DB Schema 8007
EN 15804: 2012-04 + A1 2014: Sustainability of
construction works — Environmental Product Institut Bauen und Umwelt
Declarations — Core rules for the product category of Institut Bauen und Umwelt e.V., Berlin(pub.): General
construction products Instructions for the EPD Programme of Institut Bauen
und Umwelt e.V., Version 2.0 2021
CEN/TR 15941
CEN/TR 15941: Sustainability of construction works - Product Category Rules for Building-Related
Environmental product declarations - Methodology for Products and Services
selection and use of generic data Institute Construction and Environment e.V. (IBU)
Part A: Calculation Rules for the Life Cycle
CEN TS 16516 Assessment and Requirements on the Project Report
CEN TS 16516: /AgBB/, /ISO 16000-3/, /ISO 16000-6/, Version 1.7
/ISO16000-9/, /ISO 16000-11/ Construction products -
Assessment of release of dangerous substances. PCR Guidance-Texts for Building-Related Products
Determination of emissions into indoor air and Services
From the range of Environmental Product Declarations
EN 16783 of Institute Construction and Environment e.V. (IBU)
EN 16783: 2017 Thermal insulation products - Product Part B: Requirements on the EPD for Insulating
category rules (PCR) for factory made and in-situ materials made of foam plastics
formed products for preparing environmental product Version 1.6 (Template) Version 1.2 (PCR specific)
declarations
Sphera
Eurostat Sphera Solutions Gmbh. GaBi 10 LCI documentation.
European Statistics: Recovery rates for packaging GaBi Databases (sphera.com) Stuttgart,
waste Paper and cardboard packaging for the Echterdingen: Sphera Solutions Gmbh
European Union 27 countries 2014
http://ec.europa.eu/eurostat/home
Eurofins
9 Environmental Product Declaration NMC sa – CLIMAFLEX®naturefoam stabil
Publisher
Institut Bauen und Umwelt e.V. Tel +49 (0)30 3087748- 0
Panoramastr. 1 Fax +49 (0)30 3087748- 29
10178 Berlin Mail info@ibu-epd.com
Germany Web www.ibu-epd.com
Programme holder
Institut Bauen und Umwelt e.V. Tel +49 (0)30 - 3087748- 0
Panoramastr 1 Fax +49 (0)30 – 3087748 - 29
10178 Berlin Mail info@ibu-epd.com
Germany Web www.ibu-epd.com
Author of the Life Cycle
Assessment Tel +32 (0) 87 85 85 00
NMC S.A. Fax +32 (0) 87 85 85 11
Gerd-Noël-Strasse 1 Mail info@nmc.eu
4731 Eynatten Web www.nmc.eu
Belgium
Owner of the Declaration
NMC S.A. Tel +32 (0) 87 85 85 00
Gerd-Noël-Strasse 1 Fax +32 (0) 87 85 85 11
4731 Eynatten Mail info@nmc.eu
Belgium Web www.nmc.eu
