ENVIRONMENTAL PRODUCT DECLARATION
as per ISO 14025 and EN 15804+A1
Owner of the Declaration NMC S.A.
Programme holder Institut Bauen und Umwelt e.V. (IBU)
Publisher Institut Bauen und Umwelt e.V. (IBU)
Declaration number EPD-NMC-20210310-IBD1-EN
Issue date 05.01.2022
Valid to 04.01.2027
CLIMAFLEX®naturefoam
NMC S.A.
www.ibu-epd.com | https://epd-online.com
Umwelt Produktdeklaration Name des Herstellers – Name des Produkts
1. General Information
NMC S.A. CLIMAFLEX®naturefoam
Programme holder Owner of the declaration
IBU – Institut Bauen und Umwelt e.V. NMC S.A.
Panoramastr. 1 Gert-Noel Strasse
10178 Berlin BE-4731 Eynatten
Germany
Declaration number Declared product / declared unit
EPD-NMC-20210310-IBD1-EN 1 m³ insulation material CLIMAFLEX®naturefoam
This declaration is based on the product Scope:
category rules: Product line CLIMAFLEX®naturefoam
Insulating materials made of foam plastics, 01.2019 Thermal insulation products for building equipment and
(PCR checked and approved by the SVR) industrial insulations made of polythene [BSJ1] foam
(PEF) according to EN14313, describing the specific
environmental performance of the product produced in
Issue date
Belgium at the site of Eynatten
05.01.2022
The owner of the declaration shall be liable for the
Valid to
underlying information and evidence; the IBU shall not
04.01.2027
be liable with respect to manufacturer information, life
cycle assessment data and evidences.
The EPD was created according to the specifications
of EN 15804+A1. In the following, the standard will be
simplified as EN 15804.
Verification
The standard EN 15804 serves as the core PCR
Independent verification of the declaration and data
according to ISO 14025:2010
Dipl. Ing. Hans Peters internally x externally
(chairman of Institut Bauen und Umwelt e.V.)
Dr. Alexander Röder Vito D'Incognito
(Managing Director Institut Bauen und Umwelt e.V.)) (Independent verifier)
2. Product
2.1 Product description/Product definition is recycled. 50 years is the minimum Reference
CLIMAFLEX®naturefoam Polyethylene foams have Service Life recommended in prEN16783 “PCR for
many environmental benefits, having a low density factory made thermal insulation products”.
(average 22 kg/m³), few raw materials are required for
the manufacture of an article and the environmental 2.3 Technical Data
impact of their transport is lower than similar articles of Performance data of the product in accordance with
higher density performing the same function. the Declaration of Performance with respect to its
Furthermore, the CLIMAFLEX®naturefoam are fully Essential Characteristics according to /EN 14313/
recyclable. apply. Further data:
For the placing on the market of the product in the
European Union/European Free Trade Association Constructional data
(EU/EFTA )(with the exception of Switzerland) - Performance data of the product in accordance with
Thermal Insulation products for building equipment and the Declaration of Performance with respect to its
industrial installations. Factory made polyethylene Essential Characteristics according to /EN 14313/
foam (PEF) and the CE-marking. For the application apply. Further data:
and use the respective national provisions apply. Name Value Unit
2.2 Application Gross density 22 kg/m3
The function of CLIMAFLEX®naturefoam is to insure 0.036 -
Thermal conductivity W/(mK)
the insulation of heating and sanitary installations for a 0.048
reference service life (RSL) of 50 years. Reaction to Fire Acc.to /EN Bl-s1d0 ;
-
This duration is based on the frequency of replacement 13501-1/ Cl-s1d0
of sanitary and heating piping in buildings. Although Max Service Temperature Acc. to
100 °C
the insulation pipes are still effective after 50 years, it /EN 14707
is assumed that when replacing the piping, the Min Service Temperature 0 °C
insulation CLIMAFLEX®naturefoam is not reused and
2 Environmental Product Declaration NMC sa – CLIMAFLEX®naturefoam
Water absorption Acc. to EN and put on the market by NMC do need to be
WS005
13472 registered. CLIMAFLEX®naturefoam do not contain
Traces quantities of water soluble Cl < 10 – F Substances of Very High Concern (SVHC). Antimony
ions and pH-value Acc. to EN < 4 - pH trioxide and halogenated flame retardants are used.
13472 and EN 13468 6,8
2.6 Manufacture
The manufacturing process consists of a continuous
2.4 Delivery status extrusion. Solid pellets of thermoplastic resin are fed
The CLIMAFLEX®naturefoam product is a closed-cell into a melting zone in which the resin is melted, to
bio-polyethylene foam insulation tube designed for form a flowable thermoplastic mass. The thermoplastic
applications in heating and sanitary installations. The mass is then metered to a mixing zone where it is
CLIMAFLEX®naturefoam range extends from 5 to 25 thoroughly mixed with a blowing agent under pressure.
mm thick and from 12 to 114mm inside diameter. They The mixture of thermoplastic resin and blowing agent
are delivered in lengths of 2 m packed in cardboard. is then forced through a die, which imparts a shape to
(More information on ranges and dimensions on the thermoplastic mass, into a zone of lower pressure
www.nmc-insulation.com.) (i.e. atmospheric pressure). The blowing agent
expands to form the cells of the foam and the
thermoplastic foam is cooled through an inline water
2.5 Base materials/Ancillary materials cooler. At the end of the inline cooler the profiles are
cut to the required dimensions.
Base materials
CLIMAFLEX®naturefoam are flexible insulation Quality assurance :
materials based on bio-polyethene, which is produced The manufacture is certified ISO 9001 for the quality
using a mixture of up to eight basic component management and the product is certified for CE
materials. The following table displays an average marking according to the CPR (CE Certificate of
weighted of different elements of the formulation, and conformity N° 0749-CPR-BC1-571-4133-0001-01and
this for the complete CLIMAFLEX®naturefoam product 0749-CPR-BC1-571-4133-0002-01)
range. The following table displays the different
elements of the formulation for
CLIMAFLEX®naturefoam. This is in accordance with 2.7 Environment and health during
the PCR Part B: Requirements on the EPD for manufacturing
Insulating materials made of foam plastics and ISO During all manufacturing steps of NMC S.A. Belgium,
14025. the production follows all national guidelines and
This product contains substances listed in the regulations. Solar panels are installed on the roof of
candidate list (date: 08.07.2021) exceeding 0.1 the warehouse and in the field to reduce the
percentage by mass: No. requirement for grid electricity.
This product contains other CMR substances in
categories 1A or 1B, which are not on the candidate 2.8 Product processing/Installation
list, exceeding 0.1 percentage by mass: No. CLIMAFLEX®naturefoam can be installed using basic
Biocide products were added to this construction tools (e.g. craft knives). No special tools, nor specific
product or it has been treated with biocide products protection is necessary. When applying adhesives the
(this then concerns a treated product as defined by the information given in the relevant safety data sheets is
(EU) Ordinance on Biocide Products No. to be heeded.
528/2012): No. Any glue and adhesive tapes used during the
installation phase were not included in the
LCA. Recommendations on how to use the product are
Name Value Unit described in the application manuals or videos. More
Bio LDPE 50,0 % details are listed on the Web Page www.nmc-
LLDPE 20,6 % insulation.com
NMC Internally recycled PE 8,8 %
Flame retardant 3,5 % 2.9 Packaging
CLIMAFLEX®naturefoam products are packed in
Pigments and fillers 3,7 %
cardboard boxes and transported on reusable pallets.
Volume stabilizer 1,8 %
All packaging material can be recycled. The pallets
Blowing Agent 11,6 %
used to transport the products are taken back or
exchanged when the CLIMAFLEX®naturefoam easy is
BIO-PE and fillers are the main components of the
delivered, so the use of pallets is a close loop
product and are responsible for the characteristics and
economy
performance of the product
The blowing agent causes the expansion during
manufacturing. The flame retardant ensures the fire
2.10 Condition of use
resistance and conformity with fire protection
During the use of the products for the purpose for
regulations (see section 2.13).
which they are intended, there are no modifications
According the European Chemicals Regulation
unless one of the effects listed in extraordinary impacts
“REACH” manufacturers, importers and downstream
occurs (see point 2.13).
users must register their chemicals and are
responsible for their safe use. NMC S.A. uses
exclusively verifiably registered and approved
substances in its production. Products manufactured
3 Environmental Product Declaration NMC sa – CLIMAFLEX®naturefoam
2.11 Environment and health during use any fire event. There is no possibility of the material
There are no particular effects on environmental and self-igniting. CLIMAFLEX®naturefoam does not
health impacts during use related to the material propagate the fire horizontally or vertically. The smoke
composition of the product. The development in case of fire is very low (class S1).
CLIMAFLEX®naturefoam products are used in a wide
range of applications across the building sector.
The PEF foams fulfil the German, Belgian and French
regulations regarding the emission of VOC with Fire protection
emissions far below the most stringent limit values. Name Value
The Eurofin Product Testing institute, at the request of Building material class Bl / Cl
the CEFEP (European group of PEF and FEF Burning droplets d0
manufacturers) has made a wide range of tests for Smoke gas development S1
different PEF products from different manufacturers.
Water
The insulation of heating pipes with CLIMAFLEX®naturefoam is a closed cell foam and
CLIMAFLEX®naturefoam allows a reduction of energy obtain the best water absorption class WS005
dispersion and of course CO 2 emissions during the full according to the product standard
service life of the installation. The quantification of this
in-use benefit is not within the scope of this EPD,
however, this could be calculated using an LCA for the Mechanical destruction
complete pipe/insulation system, and has to be CLIMAFLEX®naturefoam is chemically inert and does
evaluated in the frame of the LCA from the complete not present any environmental or health risk if
heating installation. A software program available on mechanically destructed. CLIMAFLEX®naturefoam is
NMC’s website http://cit.nmc-insulation.com/ allows for not UV resistant. The product is not recommended for
the calculation of the heat flow and insulation benefit outside applications without complementary UV
under real use conditions. protection
2.12 Reference service life 2.14 Re-use phase
The function of CLIMAFLEX®naturefoam is to ensure In principle, if removed carefully,
the insulation of heating and sanitary installations for a CLIMAFLEX®naturefoam can be reused on any other
reference service life (RSL) of 50 years. This duration piping system of similar dimensions. Any material not
is based on the frequency of replacement of sanitary suitable for reuse is fully recyclable.
and heating piping in buildings. Although the insulation
pipes are still effective after 50 years, it is assumed 2.15 Disposal
that when replacing the piping, the insulation The CLIMAFLEX®naturefoam is fully recyclable and
(CLIMAFLEX®naturefoam ) is recycled. 50 years is the can be used as a direct one-for-one substitute for
minimum Reference Service Life recommended in virgin PE-LD granulates, with only minor additive
/EN16783/ “PCR for factory made thermal insulation additions. There is no chemical difference between
products”. bio-based PE-LD and fossil fuel derived PE-LD, so
using a mix of sources does not change the
recyclability of the product.
2.13 Extraordinary effects
2.16 Further information
Fire Additional information about
According to CLIMAFLEX®naturefoam is classified as CLIMAFLEX®naturefoam can be found on the NMC
a combustible insulation material. Due to its material web site www.nmc-insulation.com Here specification
structure, CLIMAFLEX®naturefoam does not clauses, data sheets and application manuals can be
contribute to an uncontrollable spread of fire under found.
installation conditions typical on a building site. The
product is self-extinguishing reducing its contribution to
3. LCA: Calculation rules
3.1 Declared Unit linear meter m3
The declared unit for insulating materials made of foam divided
plastic is 1 m³. The EPD will cover the section of
whole CLIMAFLEX®naturefoam range. The insulating the
sleeves in the CLIMAFLEX®naturefoam range have a insulation
thickness ranging from 5 to 25mm and an inside pipe ( m²)
diameter ranging from 12 to 114mm The average Thermal Conductivity λ : 0.040 W/mK at (40°C)
reference density of CLIMAFLEX®naturefoam is 22 R-value- thickness- : 25 mm : +/- 3.5 (m²K/W)
kg/m³. depending on the pipe diameter.
Declared unit
Name Value Unit 3.2 System boundary
Declared unit 1 m3 The Data collection refers to the yearly production in
Gross density 22 kg/m3 2020.
Volume for 1kg 0.0455 m³
Conversion factor from 1 m³ to 1 Value for 1 m
4 Environmental Product Declaration NMC sa – CLIMAFLEX®naturefoam
Module A1 to A3: The LCA calculation covers the additive additions. There is no chemical difference
production of the raw materials, transport of these to between bio-based PE-LD and fossil fuel derived PE-
the plant, the mixing of raw materials according to the LD, so using a mix of sources does not change the
respective recipes, manufacturing of the foam product recyclability of the product.
and packaging for dispatch. All production takes place
exclusively in Eynatten, Belgium. 3.3 Estimates and assumptions
The LCA calculation is conducted using the Gabi ts -
Module A4: NMC’s logistics department reported database. Not all necessary LCIs are included in the
average figures for the distribution of NMC’s products - database. Where data were missing or were
depending on the country the transport distance unavailable or where suppliers were unable to provide
varies. The biggest customers represent 78,7% of complete information, proxy datasets have been used.
sales volumes in 2020, with the remainder supplied to The environmental burden for the production of
a large set of smaller customers. pigments, flame retardants and volume stabilizers are
approximated.
Module A5: Installation of CLIMAFLEX®naturefoam
products is done by hand and requires no special
equipment apart from a knife. The products can be 3.4 Cut-off criteria
placed end to end and the remaining pieces can be Any glue and adhesive tapes used during the
reused. Some glue or tape could be used for the installation (A5) have not been included as
installation, as the quantity or the product used quantification of these materials is uncertain and their
depends on the final customer, he has to calculate the use by the various installers is too diverse, adhesives
impact of what he used himself. The environmental and glues are not required in all/most cases, but may
impact of this type of accessory is not counted in this be used for some applications.
study. The calculations do not contain any installation In this study no others cut-off criteria have been
waste. Cardboard as packaging material is assumed to applied and all elementary incoming processes as well
be recycled. As input material cardboard made of as all energy and water inputs and waste outputs have
waste paper is considered. Thus, environmental been counted.
burden for packaging material are considered already
in A1-A3. The value of the environmental impact for A5 3.5 Background data
is declared as “0”. The choice made is : the final user The software system for life cycle engineering /GaBi
has to calculate the impact of A5 himself in the function 10/ developed by thinkstep AG was used to perform
of his own case, by accounting for the extra amount of this LCA. The GaBi LCI database /GaBi 10/ provides
product needed during installation. the life cycle inventory data for several of the raw and
process materials obtained from the background
Module B1-B7:Once installed the system. The most recent update of the database was
CLIMAFLEX®naturefoam product requires no in 2020.
maintenance and no repair. It will be dismantled when
the sanitary pipe is replaced. For this reason, there are 3.6 Data quality
not expected to be any impacts in B1 to B7 assuming All the foreground data requiring such energy or raw
correct specification and installation.The step B1 is not material coming from production, were verified and
considered in this LCA, although the insulation of the cross-checked before being included in the model.
piping contributes to a significant reduction of CO2 Most of the life cycle inventories for the basic materials
emissions from the heating or cooling equipment, this are available in the/ GaBi 10/ database.
is not taken into account in this LCA. It should, For electrical and thermal energy Belgium specific grid
however, be taken into account in the calculation of mixes and Belgium specific supply for natural gas were
environmental impacts of the complete heating and considered.
cooling systems or of the complete building.
3.7 Period under review
Module C1: As for the installation of the product, the The production data for the year 2020 were used for
disassembly is done manually and does not require the realization of this study.
any specific equipment. Disassembly is generally
carried out at the same time as the replacement or 3.8 Allocation
removal of sanitary pipes. Consequently, there are no There is no co-product or by-product generated during
impacts associated with C1. the production of NMC’s products.
Module C2: Transport at end-of-life stage is modeled Due to the lack of specific data per production line and
as a Euro Cargo 0-6 mix truck with diesel fuel. The product, the energy has been allocated per overall
average distance to either mechanical recycling, produced volume of insulation foam.
incineration or landfills is assumed to be 100 km
Production waste
Module C3:The scenario that has been retained for Most of the production waste from the process
this Life Cycle Assessment is the 100% recycling (machine start, end of production, non-conforming
scenario. products, etc.) is recycled internally in order to be
reused in the manufacturing process. These impacts
Module C4: As CLIMAFLEX®naturefoam is fully are accounted for in A1-A3.
recyclable, the legislation is pushing more in this
direction and the overall pressure on plastic recycling Installation and End-of-Life waste
is growing, the scenario with recycling is considered. Installation of the foam products is done by hand and
requires no special equipment apart from a knife.
Module D:The CLIMAFLEX®naturefoam is fully Installation off-cut is not considered in this calculations.
recyclable and can be used as a direct one-for-one Any glue and adhesive tapes used during the
substitute for virgin PE-LD granulates, with only minor installation phase were not included in the LCA.
5 Environmental Product Declaration NMC sa – CLIMAFLEX®naturefoam
3.9 Comparability
Basically, a comparison or an evaluation of EPD data
is only possible if all the data sets to be compared
were created according to EN 15804 and the building
context, respectively the product-specific
characteristics of performance, are taken into account.
4. LCA: Scenarios and additional technical information
Name Value Unit
Reference service life years 50 a
Transport to the building site (A4)
Name Value Unit
Litres of fuel 0.096 l/100km Operational energy use (B6) and Operational water
Transport distance 487 km use (B7)
Capacity utilisation (including Name Value Unit
10 %
empty runs) Water consumption - m3
Gross density of products Electricity consumption - kWh
22 kg/m3
transported Other energy carriers - MJ
Equipment output - kW
Installation into the building (A5)
Name Value Unit End of life (C1-C4)
Name Value Unit
Recycling 22 kg
Use or application of the installed product (B1) see
section 2.12 "Use" Reuse, recovery and/or recycling potentials (D),
Name Value Unit relevant scenario information
One of the benefits beyond the boundaries of the
Maintenance (B2) system is the recyclability of the Climaflex product.
Name Value Unit Recycled PE-LD granulate can be used as a substitute
Information on maintenance - - for virgin PE-LD granulate on a one-for-one basis.
Number/ Furthermore, there are no differences in the properties
Maintenance cycle -
RSL or performance of bio-based PE-LD and PE-LD
Water consumption - m3 derived from fossil fuels. It is assumed that recycled
Auxiliary - kg granulate generated from Climaflex products displace
Other resources - kg the need for fossil fuel derived PE-LD granulate.
Electricity consumption - kWh
Other energy carriers - MJ Another benefit beyond the boundaries of the system
Material loss - kg is the recovery of energy generated from the
incineration of waste at end-of-life. This is modeled in
Repair (B3) the GaBi7 software using an industry-average dataset
Name Value Unit for the incineration of polyethylene and according to
Information on the repair process - - the quantity of waste at end-of-life. The recovery of
Information on the inspection process - - thermal and electrical energy produced by the
Number/ incinerator avoids the use of fossil resources.
Repair cycle -
RSL
Water consumption - m3 Name Value Unit
Auxiliary - kg
Other resources - kg
Electricity consumption - kWh
Other energy carriers - MJ
Material loss - kg
Replacement (B4) / Refurbishment (B5)
Name Value Unit
Number/
Replacement cycle -
RSL
Electricity consumption - kWh
Litres of fuel - l/100km
Replacement of worn parts - kg
Reference service life
6 Environmental Product Declaration NMC sa – CLIMAFLEX®naturefoam
5. LCA: Results
DESCRIPTION OF THE SYSTEM BOUNDARY (X = INCLUDED IN LCA; MND = MODULE NOT DECLARED;
MNR = MODULE NOT RELEVANT)
BENEFITS AND
CONSTRUCTI LOADS
PRODUCT STAGE ON PROCESS USE STAGE END OF LIFE STAGE BEYOND THE
STAGE SYSTEM
BOUNDARIES
7 Environmental Product Declaration NMC sa – CLIMAFLEX®naturefoam
lairetam
waR
ylppus tropsnarT
gnirutcafunaM
eht
morf
tropsnarT
etis
eht
ot
etag
ylbmessA esU
ecnanetniaM
riapeR
tnemecalpeR tnemhsibrufeR
ygrene
lanoitarepO esu
retaw
lanoitarepO esu
noitcurtsnoc-eD
noitilomed tropsnarT
gnissecorp
etsaW
lasopsiD -esueR -yrevoceR -gnilcyceR laitnetop
A1 A2 A3 A4 A5 B1 B2 B3 B4 B5 B6 B7 C1 C2 C3 C4 D
X X X X X MND MND MNR MNR MNR MND MND MND X X X X
RESULTS OF THE LCA - ENVIRONMENTAL IMPACT according to EN 15804+A1: 1 m³ CLIMAFLEX®
naturefoam
Parameter Unit A1-A3 A4 A5 C2 C3 C4 D
GWP [kg CO2-Eq.] 19.88 0.94 0.00 0.13 1.42 0.00 -40.12
ODP [kg CFC11-Eq.] 1.53E-8 2.52E-16 0.00E+0 3.51E-17 1.28E-13 0.00E+0 -5.32E-13
AP [kg SO2-Eq.] 4.71E-1 8.05E-4 0.00E+0 1.12E-4 1.47E-3 0.00E+0 -4.57E-2
EP [kg (PO4)3--Eq.] 4.12E-1 1.61E-4 0.00E+0 2.25E-5 3.57E-4 0.00E+0 -7.19E-3
POCP [kg ethene-Eq.] 1.24E-1 1.05E-4 0.00E+0 1.46E-5 1.70E-4 0.00E+0 -8.11E-3
ADPE [kg Sb-Eq.] 9.03E-2 8.49E-8 0.00E+0 1.18E-8 1.06E-6 0.00E+0 -9.70E-6
ADPF [MJ] 1030.74 12.61 0.00 1.76 18.86 0.00 -1553.17
GWP = Global warming potential; ODP = Depletion potential of the stratospheric ozone layer; AP = Acidification potential of land and water; EP =
Caption Eutrophication potential; POCP = Formation potential of tropospheric ozone photochemical oxidants; ADPE = Abiotic depletion potential for non-
fossil resources; ADPF = Abiotic depletion potential for fossil resources
RESULTS OF THE LCA - INDICATORS TO DESCRIBE RESOURCE USE according to EN 15804+A1: 1 m³
CLIMAFLEX® naturefoam
Parameter Unit A1-A3 A4 A5 C2 C3 C4 D
PERE [MJ] 1053.19 0.73 0.00 0.10 19.09 0.00 -97.70
PERM [MJ] 517.79 0.00 0.00 0.00 0.00 0.00 0.00
PERT [MJ] 1570.98 0.73 0.00 0.10 19.09 0.00 -97.70
PENRE [MJ] 975.69 12.78 0.00 1.78 57.14 0.00 -1585.58
PENRM [MJ] 268.17 0.00 0.00 0.00 0.00 0.00 0.00
PENRT [MJ] 1243.86 12.78 0.00 1.78 57.14 0.00 -1585.58
SM [kg] 10.41 0.00 0.00 0.00 0.00 0.00 0.00
RSF [MJ] 0.00 0.00 0.00 0.00 0.00 0.00 0.00
NRSF [MJ] 0.00 0.00 0.00 0.00 0.00 0.00 0.00
FW [m³] 0.17 0.00 0.00 0.00 0.01 0.00 -0.18
PERE = Use of renewable primary energy excluding renewable primary energy resources used as raw materials; PERM = Use of
renewable primary energy resources used as raw materials; PERT = Total use of renewable primary energy resources; PENRE = Use of
non-renewable primary energy excluding non-renewable primary energy resources used as raw materials; PENRM = Use of non-
Caption
renewable primary energy resources used as raw materials; PENRT = Total use of non-renewable primary energy resources; SM = Use
of secondary material; RSF = Use of renewable secondary fuels; NRSF = Use of non-renewable secondary fuels; FW = Use of net fresh
water
RESULTS OF THE LCA – WASTE CATEGORIES AND OUTPUT FLOWS according to EN 15804+A1:
1 m³ CLIMAFLEX® naturefoam
Parameter Unit A1-A3 A4 A5 C2 C3 C4 D
HWD [kg] 1.30E-4 6.74E-10 0.00E+0 9.38E-11 1.95E-8 0.00E+0 -2.33E-7
NHWD [kg] 5.70E+0 2.01E-3 0.00E+0 2.79E-4 6.24E-2 0.00E+0 -4.33E-1
RWD [kg] 6.22E-2 2.32E-5 0.00E+0 3.23E-6 1.51E-2 0.00E+0 -1.22E-2
CRU [kg] 0.00 0.00 0.00 0.00 0.00 0.00 0.00
MFR [kg] 0.00 0.00 10.41 0.00 22.00 0.00 0.00
MER [kg] 0.00 0.00 0.00 0.00 0.00 0.00 0.00
EEE [MJ] 0.00 0.00 0.00 0.00 0.00 0.00 0.00
EET [MJ] 0.00 0.00 0.00 0.00 0.00 0.00 0.00
HWD = Hazardous waste disposed; NHWD = Non-hazardous waste disposed; RWD = Radioactive waste disposed; CRU = Components
Caption for re-use; MFR = Materials for recycling; MER = Materials for energy recovery; EEE = Exported electrical energy; EET = Exported
thermal energy
6. LCA: Interpretation
The base polymer used at NMC is produced from advantages of using a biopolymer is a significant
renewable raw materials (Biomass). One of the reduction in greenhouse gas emissions compared to
the use of raw material of fossil origin. In addition, the As the CLIMAFLEX®naturefoam is fully recyclable; the
use of non-renewable raw materials is avoided in this choice for the end of life was that of 100% recycling.
way. This avoids the use of new raw materials and or the
When we analyse the complete life cycle we see that exploitation of renewable or non-renewable resources.
the most impacting part for all environmental impact One way to continue to reduce the environmental
factors is the production module and more particularly impact of the CLIMAFLEX®naturefoam would be to
the raw materials. With regard to global warming for continue to diversify our energy sources by switching
the complete life cycle, more than 83% comes from the more and more to renewable energies. One way to
production module 2.1% of transport to the places of continue to reduce the environmental impact of the
installation and 14.3% comes from the end of life. For CLIMAFLEX® naturefoam would be to continue to
all other impact factors, more than 90% of the impacts diversify our energy sources by switching more and
come from the production phase. more to renewable energies. To this end, after having
Transport has a more pronounced impact on global greatly increased the number of photovoltaic panels,
warming potential as well as on soil and water NMC will acquire a cogeneration system. Looking for
acidification potential and abiotic fossil resource more eco-responsible suppliers must also be put in
depletion potential. A more in-depth analysis of the place, as well as finding raw materials manufactured
production module A1 to A3 shows that the production locally to avoid long-distance transport as much as
of raw materials and their transport account for almost possible.
80% of the impact Global Warming Potential.
7. Requisite evidence
7.1. VOC emissions Sum SVOC (C16 - C22) - μg/m3
Eurofins Product Testing A/S has tested a wide range R (dimensionless) - -
and variety of typical PEF (Polyethylene foam) VOC without NIK - μg/m3
products marketed in the EU from CEFEP (European Carcinogenic Substances - μg/m3
Group of PEF/FEF manufacturers) Based on the
loading factor 0.05m²/m3 (determined after AgBB overview of results (3 days [µg/m³])
consideration of the real life applications of PEF Name Value Unit
products (in living rooms) and recommendations by the TVOC (C6 - C16) - μg/m3
experts of the test institute) all results were found to be Sum SVOC (C16 - C22) - μg/m3
clearly below the limit values. For all samples below
R (dimensionless) - -
100mg/m3 TVOC after 28 days. Certificates are
VOC without NIK - μg/m3
available on request.
Carcinogenic Substances - μg/m3
7.2 Leaching
VOC Emissions
According to /EN 13468/ the content of water-soluble
Name Value Unit
chloride ions for CLIMAFLEX®naturefoam is <10mg/kg
Overview of Results (28 Tage) - μg/m3
TVOC (C6 - C16) - μg/m3
8. References
EN 1602
EN 1602: 2013: Thermal insulating products for ISO 14040
building applications - Determination of the apparent ISO 14040: Environmental management — Life cycle
density assessment — Principles and framework
EN ISO 8497 ISO 14044
EN ISO 8497: Thermal insulation - Determination of ISO 14044: Environmental management — Life cycle
steady-state thermal transmission properties of thermal assessment — Requirements and guidelines
insulation for circular pipes
EN 14707
ISO 9001 EN 14707: 2012: Thermal insulating products for
ISO 9001: 2015: Quality management systems. building equipment and industrial installations.
Determination of maximum service temperature for
EN 13501-1 preformed pipe insulation
EN 13501-1:2007+A1: 2013 Fire classification of
construction products and building elements - EN 15804
Classification using test data from reaction to fire tests EN 15804: 2012-04 + A1 2014: Sustainability of
construction works — Environmental Product
ISO 14001 Declarations — Core rules for the product category of
ISO 14001: 2015 Environmental management construction products
systems.
CEN/TR 15941
EN ISO 14025 CEN/TR 15941: Sustainability of construction works -
EN ISO 14025: 2011-10: Environmental labels and Environmental product declarations - Methodology for
declarations — Type III environmental declarations — selection and use of generic data
Principles and procedures
8 Environmental Product Declaration NMC sa – CLIMAFLEX®naturefoam
CEN TS 16516 Instructions for the EPD Programme of Institut Bauen
CEN TS 16516: /AgBB/, /ISO 16000-3/, /ISO 16000-6/, und Umwelt e.V., Version 2.0 2021
/ISO16000-9/, /ISO 16000-11/ Construction products -
Assessment of release of dangerous substances. Product Category Rules for Building-Related
Determination of emissions into indoor air Products and Services
Institute Construction and Environment e.V. (IBU)
EN 16783 Part A: Calculation Rules for the Life Cycle
EN 16783: 2017 Thermal insulation products - Product Assessment and Requirements on the Project Report
category rules (PCR) for factory made and in-situ Version 1.7
formed products for preparing environmental product
declarations PCR Guidance-Texts for Building-Related Products
and Services
Eurostat From the range of Environmental Product Declarations
European Statistics: Recovery rates for packaging of Institute Construction and Environment e.V. (IBU)
waste Paper and cardboard packaging for the Part B: Requirements on the EPD for Insulating
European Union 27 countries 2014 materials made of foam plastics
http://ec.europa.eu/eurostat/home Version 1.6 (Template) Version 1.2 (PCR specific)
Eurofins Sphera
Eurofins: Product Testing Institute Sphera Solutions Gmbh. GaBi 10 LCI documentation.
GaBi Databases (sphera.com) Stuttgart,
Gabi ts Echterdingen: Sphera Solutions Gmbh
GaBi 10 GaBi Software-System and Database for Life
Cycle Engineering Copyright © 1992-2021 Sphera
Solutions Gmbh Version: 10.5.0.78 DB Schema 8007
Institut Bauen und Umwelt
Institut Bauen und Umwelt e.V., Berlin(pub.): General
9 Environmental Product Declaration NMC sa – CLIMAFLEX®naturefoam
Publisher
Institut Bauen und Umwelt e.V. Tel +49 (0)30 3087748- 0
Panoramastr. 1 Fax +49 (0)30 3087748- 29
10178 Berlin Mail info@ibu-epd.com
Germany Web www.ibu-epd.com
Programme holder
Institut Bauen und Umwelt e.V. Tel +49 (0)30 - 3087748- 0
Panoramastr 1 Fax +49 (0)30 – 3087748 - 29
10178 Berlin Mail info@ibu-epd.com
Germany Web www.ibu-epd.com
Author of the Life Cycle
Assessment Tel +32 (0) 87 85 85 00
NMC S.A. Fax +32 (0) 87 85 85 11
Gerd-Noël-Strasse 1 Mail info@nmc.eu
4731 Eynatten Web www.nmc.eu
Belgium
Owner of the Declaration
NMC S.A. Tel +32 (0) 87 85 85 00
Gerd-Noël-Strasse 1 Fax +32 (0) 87 85 85 11
4731 Eynatten Mail info@nmc.eu
Belgium Web www.nmc.eu
