Environmental product declaration
in accordance with ISO 14025 and EN 15804+A2
COEX-RG Cable pipe
Owner of the declaration: Program operator:
Hallingplast AS The Norwegian EPD Foundation
Product: Declaration number:
COEX-RG Cable pipe
NEPD-8440-7672-EN
Declared unit:
1 kg Registration number:
This declaration is based on Product Category Rules: NEPD-8440-7672-EN
CEN Standard EN 15804:2012+A2:2019 serves as core
Issue date: 11.12.2024
PCR
The Norwegian EPD Foundation NPCR 028:2020 Part B for Cable pipes Valid to: 11.12.2029
EPD software:
LCAno EPD generator ID: 547354
1 / 11
General information
Product Owner of the declaration:
COEX-RG Cable pipe Hallingplast AS
Contact person: Guro L. Lilleslåtten
Phone: +47 32 09 55 99
e-mail: post@hallingplast.no
Program operator: Manufacturer:
The Norwegian EPD Foundation Hallingplast AS
Post Box 5250 Majorstuen, 0303 Oslo, Norway
Phone: +47 977 22 020
web: www.epd-norge.no
Declaration number: Place of production:
Hallingplast AS
NEPD-8440-7672-EN
Kleivi næringspark 4
3570 Ål, Norway
This declaration is based on Product Category Rules: Management system:
CEN Standard EN 15804:2012+A2:2019 serves as core PCR NS-EN ISO 9001 : 2015
NPCR 028:2020 Part B for Cable pipes
Statement of liability: Organisation no:
The owner of the declaration shall be liable for the underlying 919 522 461
information and evidence. EPD Norway shall not be liable with respect
to manufacturer information, life cycle assessment data and
evidences.​
Declared unit: Issue date:
1 kg COEX-RG Cable pipe 11.12.2024
Declared unit with option: Valid to:
A1-A3,A4,A5,C1,C2,C3,C4,D 11.12.2029
Year of study:
2022
Functional unit: Comparability:
Not applicable EPD of construction products may not be comparable if they not
comply with EN 15804 and seen in a building context.
General information on verification of EPD from EPD tools: Development and verification of EPD:
Independent verification of data, other environmental information The declaration is created using EPD tool lca.tools ver EPD2022.03,
and the declaration according to ISO 14025:2010, § 8.1.3 and § 8.1.4. developed by LCA.no. The EPD tool is integrated in the company's
Verification of each EPD is made according to EPD-Norway’s management system, and has been approved by EPD Norway.
guidelines for verification and approval requiring that tools are i) NEPDT83
integrated into the company's environmental management system, ii)
the procedures for use of the EPD tool are approved by EPD-Norway, Developer of EPD: Tore Gjeldokk
and iii) the process is reviewed annually by an independent third
Reviewer of company-specific input data and EPD:​ Jonas Hegerholm
party verifier. See Appendix G of EPD-Norway's General Programme
Instructions for further information on EPD tools
Verification of EPD tool: Approved:
Independent third party verification of the EPD tool, background data
and test-EPD in accordance with EPDNorway's procedures and
guidelines for verification and approval of EPD tools. Approval
number: NEPDT49.
Third party verifier:
Vito D’Incognito, Take Care International
(no signature required)
2 / 11
Product
Product description:
COEX-RG Cable pipes for cable protection. These pipes can be installed above ground, in trenches, in water and with trenchless technology. The PE
pipes are coloured according to national requirements. The EPD covers both coiled pipes and pipes in straight lengths.
This EPD is for co-extruded pipe with black inner layer and red outer layer.
For project specific EPD other colours can be included.
For more information: www.hallingplast.no
Product specification
The product standard for these pipes is NS-EN 12201.
Materials kg %
Plastic - Internally recycled 0,90 90,00
Plastic - Polyethylene 0,01 1,00
Plastic - Polyethylene (HDPE) 0,09 9,00
Total 1,00 100,00
Technical data:
The material density for these products is 960 kg/m3. The dimensions given for these products, i.e. diameter and wall thickness, are mean values
based on the dimensions given in the product standard.
For additional technical information:
www.hallingplast.no
Market:
Mainly Norway.
Reference service life, product
At least 100 years if installed according to manufacturer and used according to product specifications.
Reference service life, building or construction works
According to service life of buildings.
LCA: Calculation rules
Declared unit:
1 kg COEX-RG Cable pipe
Cut-off criteria:
All major raw materials and all the essential energy is included. The production processes for raw materials and energy flows with very small
amounts (less than 1%) are not included. These cut-off criteria do not apply for hazardous materials and substances.
Allocation:
The allocation is made in accordance with the provisions of EN 15804:2012+A2:2019. Incoming energy and water and waste production in-house
is allocated equally among all products through mass allocation. Effects of primary production of recycled materials is allocated to the main
product in which the material was used. The recycling process and transportation of the material is allocated to this analysis.
Data quality:
Specific data for the product composition are provided by the manufacturer. The data represent the production of the declared product and were
collected for EPD development in the year of study. Background data is based on EPDs according to EN 15804 and different LCA databases. The
data quality of the raw materials in A1 is presented in the table below.
Materials Source Data quality Year
Plastic - Internally recycled LCA.no Database 2024
Plastic - Polyethylene ecoinvent 3.6 Database 2019
Plastic - Polyethylene (HDPE) ecoinvent 3.6 Database 2019
3 / 11
System boundaries (X=included, MND=module not declared, MNR=module not relevant)
Construction Beyond the system
Product stage Use stage End of life stage
installation stage boundaries
A1 A2 A3 A4 A5 B1 B2 B3 B4 B5 B6 B7 C1 C2 C3 C4 D
X X X X X MND MND MND MND MND MND MND X X X X X
System boundary:
Additional technical information:
ISCC (bio circular raw material) is not included in this EPD, according to regulations given by EPD Norge.
Packaging material is not included in this EPD, but can be provided for project specific EPD on request. Hallingplast AS is continously striving to
minimize the use of packaging material while delivering high quality products to the customer.
A1 has been calculated according to data from 2021, 2022 and 2023.
waR slairetam tropsnarT gnirutcafunaM tropsnarT ylbmessA e​sU ecnanetniaM riapeR tnemecalpeR tnemhsibrufeR lanoitarepO ygrene esu lanoitarepO esu retaw -eD noitcurtsnoc noitilomed tropsnarT etsaW gnissecorp lasopsiD -yrevoceR-esueR laitnetop-gnilcyceR
4 / 11
LCA: Scenarios and additional technical information
The following information describe the scenarios in the different modules of the EPD.
The system boundary for this EPD is modules A1-A4.
A4: Distance for transport from manufacturer to building site has been set to 300 km as given in the PCR.
A5: Has not been included, but can be provided for project specific EPD on request. This, due to various installation practices.
C1-C4: Is based on national statistics.
Capacity utilisation Value
Transport from production place to user (A4) Distance (km) Fuel/Energy Consumption Unit
(incl. return) % (Liter/tonne)
Truck, 16-32 tonnes, EURO 6 (km) - Europe 36,7 % 300 0,043 l/tkm 12,90
De-construction demolition (C1) Unit Value
End-of-life treatments of polyethylene (PE) cable
kg/DU 1,00
pipe for electrical cables (kg)
Capacity utilisation Value
Transport to waste processing (C2) Distance (km) Fuel/Energy Consumption Unit
(incl. return) % (Liter/tonne)
Truck, 16-32 tonnes, EURO 6 (km) - Europe 36,7 % 85 0,043 l/tkm 3,66
Waste processing (C3) Unit Value
Waste treatment per kg Polyethylene (PE),
kg 0,50
incineration with fly ash extraction (kg)
Disposal (C4) Unit Value
Landfilling of ashes from incineration of
Polyethylene (PE), process per kg ashes and kg 0,02
residues (kg)
Waste, polyethylene (PE), to landfill (kg) kg 0,50
Benefits and loads beyond the system
Unit Value
boundaries (D)
Substitution of electricity, in Norway (MJ) MJ 0,97
Substitution of thermal energy, district heating, in
MJ 14,67
Norway (MJ)
5 / 11
LCA: Results
The LCA results are presented below for the declared unit defined on page 2 of the EPD document.
Environmental impact
Indicator Unit A1-A3 A4 A5 C1 C2 C3 C4 D
GWP-total kg CO2 -eq 2,49E-01 5,03E-02 0 0,00E+00 1,42E-02 1,51E+00 7,39E-02 -8,81E-02
GWP-fossil kg CO2 -eq 2,47E-01 5,02E-02 0 0,00E+00 1,42E-02 1,51E+00 7,38E-02 -8,50E-02
GWP-biogenic kg CO2 -eq 2,10E-03 2,08E-05 0 0,00E+00 5,89E-06 1,22E-05 5,55E-06 -1,76E-04
GWP-luluc kg CO2 -eq 1,43E-04 1,79E-05 0 0,00E+00 5,07E-06 1,79E-06 1,19E-06 -2,93E-03
ODP kg CFC11 -eq 1,18E-08 1,14E-08 0 0,00E+00 3,22E-09 1,16E-09 1,66E-09 -6,20E-03
AP mol H+ -eq 1,25E-03 1,44E-04 0 0,00E+00 4,09E-05 1,89E-04 4,05E-05 -7,01E-04
EP-FreshWater kg P -eq 5,12E-06 4,01E-07 0 0,00E+00 1,14E-07 1,16E-07 6,15E-08 -7,56E-06
EP-Marine kg N -eq 2,17E-04 2,86E-05 0 0,00E+00 8,09E-06 9,07E-05 2,73E-05 -2,29E-04
EP-Terrestial mol N -eq 2,40E-03 3,19E-04 0 0,00E+00 9,05E-05 9,81E-04 1,63E-04 -2,48E-03
POCP kg NMVOC -eq 9,87E-04 1,22E-04 0 0,00E+00 3,47E-05 2,35E-04 6,24E-05 -6,83E-04
ADP-minerals&metals1 kg Sb-eq 2,99E-06 1,39E-06 0 0,00E+00 3,93E-07 5,28E-08 4,25E-08 -8,46E-07
ADP-fossil1 MJ 7,73E+00 7,59E-01 0 0,00E+00 2,15E-01 9,87E-02 1,22E-01 -1,22E+00
WDP1 m3 3,46E+01 7,35E-01 0 0,00E+00 2,08E-01 2,23E-01 8,87E-01 -1,51E+01
GWP-total = Global Warming Potential total; GWP-fossil = Global Warming Potential fossil fuels; GWP-biogenic = Global Warming Potential biogenic; GWP-luluc =
Global Warming Potential land use and land use change; ODP = Depletion potential of the stratospheric ozone layer; AP = Acidification potential, Accumulated
Exceedance; EP-freshwater = Eutrophication potential, fraction of nutrients reaching freshwater end compartment: EP-marine = Eutrophication potential, fraction of
nutrients reaching marine end compartment; EP-terrestrial = Eutrophication potential, Accumulated Exceedance; POCP = Formation potential of tropospheric ozone;
ADP-minerals&metals = Abiotic depletion potential for non-fossil resources; ADP-fossil = Abiotic depletion for fossil resources potential; WDP = Water (user)
deprivation potential, deprivation-weighted water consumption
"Reading example: 9,0 E-03 = 9,0*10-3 = 0,009"
*INA Indicator Not Assessed
1. The results of this environmental impact indicator shall be used with care as the uncertainties on these results are high or as there is limited experienced with the
indicator
Remarks to environmental impacts
Hallingplast AS is continously striving to minimize the use of packaging material while delivering high quality products to the customer.
Hallingplast AS can provide bio circular pressure pipes through ISCC certification. Contact our sales representatives for more information.
It is important that the customer handles wastes according to local regulations.
6 / 11
Additional environmental impact indicators
Indicator Unit A1-A3 A4 A5 C1 C2 C3 C4 D
PM Disease incidence 1,11E-08 3,08E-09 0 0,00E+00 8,71E-10 7,40E-10 8,22E-10 -4,25E-08
IRP2 kgBq U235 -eq 9,59E-03 3,32E-03 0 0,00E+00 9,40E-04 1,67E-04 5,71E-04 -7,77E-03
ETP-fw1 CTUe 2,34E+00 5,63E-01 0 0,00E+00 1,60E-01 2,95E-01 9,07E-02 -6,61E+00
HTP-c1 CTUh 1,41E-10 0,00E+00 0 0,00E+00 0,00E+00 3,40E-11 4,00E-12 -1,21E-10
HTP-nc1 CTUh 2,52E-09 6,15E-10 0 0,00E+00 1,74E-10 1,27E-09 9,40E-11 -6,34E-09
SQP1 dimensionless 6,33E-01 5,31E-01 0 0,00E+00 1,51E-01 1,20E-02 4,58E-01 -8,13E+00
PM = Particulate Matter emissions; IRP = Ionizing radiation – human health; ETP-fw = Eco toxicity – freshwater; HTP-c = Human toxicity – cancer effects; HTP-nc =
Human toxicity – non cancer effects; SQP = Potential Soil Quality Index (dimensionless)
"Reading example: 9,0 E-03 = 9,0*10-3 = 0,009"
*INA Indicator Not Assessed
1. The results of this environmental impact indicator shall be used with care as the uncertainties on these results are high or as there is limited experienced with the
indicator
2. This impact category deals mainly with the eventual impact of low dose ionizing radiation on human health of the nuclear fuel cycle. It does not consider effects due
to possible nuclear accidents, occupational exposure nor due to radioactive waste disposal in underground facilities. Potential ionizing radiation from the soil, from
radon and from some construction materials is also not measured by this indicator.
7 / 11
Resource use
Indicator Unit A1-A3 A4 A5 C1 C2 C3 C4 D
PERE MJ 2,11E+00 1,09E-02 0 0,00E+00 3,08E-03 2,90E-03 5,02E-03 -7,51E+00
PERM MJ 0,00E+00 0,00E+00 0 0,00E+00 0,00E+00 0,00E+00 0,00E+00 0,00E+00
PERT MJ 2,11E+00 1,09E-02 0 0,00E+00 3,08E-03 2,90E-03 5,02E-03 -7,51E+00
PENRE MJ 3,75E+00 7,59E-01 0 0,00E+00 2,15E-01 9,87E-02 1,22E-01 -1,22E+00
PENRM MJ 4,27E+00 0,00E+00 0 0,00E+00 0,00E+00 -4,16E+00 0,00E+00 0,00E+00
PENRT MJ 8,02E+00 7,59E-01 0 0,00E+00 2,15E-01 -4,06E+00 1,22E-01 -1,22E+00
SM kg 9,23E-01 0,00E+00 0 0,00E+00 0,00E+00 0,00E+00 0,00E+00 0,00E+00
RSF MJ 9,73E-03 3,89E-04 0 0,00E+00 1,10E-04 8,17E-05 1,06E-04 -1,32E-03
NRSF MJ 8,64E-03 1,39E-03 0 0,00E+00 3,94E-04 0,00E+00 1,97E-03 -4,45E-01
FW m3 1,72E-02 8,12E-05 0 0,00E+00 2,30E-05 2,79E-04 1,48E-04 -9,05E-03
PERE = Use of renewable primary energy excluding renewable primary energy resources used as raw materials; PERM = Use of renewable primary energy resources used
as raw materials; PERT = Total use of renewable primary energy resources; PENRE = Use of non renewable primary energy excluding non-renewable primary energy
resources used as raw materials; PENRM = Use of non renewable primary energy resources used as raw materials; PENRT = Total use of non renewable primary energy
resources; SM = Use of secondary materials; RSF = Use of renewable secondary fuels; NRSF = Use of non-renewable secondary fuels; FW = Net use of fresh water
"Reading example: 9,0 E-03 = 9,0*10-3 = 0,009"
*INA Indicator Not Assessed
8 / 11
End of life - Waste
Indicator Unit A1-A3 A4 A5 C1 C2 C3 C4 D
HWD kg 9,82E-04 3,92E-05 0 0,00E+00 1,11E-05 0,00E+00 1,49E-02 -5,72E-05
NHWD kg 4,06E-02 3,69E-02 0 0,00E+00 1,05E-02 0,00E+00 5,08E-01 -2,87E-02
RWD kg 8,45E-06 5,17E-06 0 0,00E+00 1,47E-06 0,00E+00 5,22E-08 -6,37E-06
HWD = Hazardous waste disposed; NHWD = Non-hazardous waste disposed; RWD = Radioactive waste disposed
"Reading example: 9,0 E-03 = 9,0*10-3 = 0,009"
*INA Indicator Not Assessed
End of life - Output flow
Indicator Unit A1-A3 A4 A5 C1 C2 C3 C4 D
CRU kg 0,00E+00 0,00E+00 0 0,00E+00 0,00E+00 0,00E+00 0,00E+00 0,00E+00
MFR kg 1,76E-03 0,00E+00 0 0,00E+00 0,00E+00 0,00E+00 0,00E+00 0,00E+00
MER kg 3,86E-03 0,00E+00 0 0,00E+00 0,00E+00 5,00E-01 0,00E+00 0,00E+00
EEE MJ 2,51E-03 0,00E+00 0 0,00E+00 0,00E+00 9,70E-01 0,00E+00 0,00E+00
EET MJ 3,80E-02 0,00E+00 0 0,00E+00 0,00E+00 1,47E+01 0,00E+00 0,00E+00
CRU = Components for re-use; MFR = Materials for recycling; MER = Materials for energy recovery; EEE = Exported energy electrical; EET = Exported energy thermal
"Reading example: 9,0 E-03 = 9,0*10-3 = 0,009"
*INA Indicator Not Assessed
Biogenic Carbon Content
Indicator Unit At the factory gate
Biogenic carbon content in product kg C 0,00E+00
Biogenic carbon content in accompanying packaging kg C 0,00E+00
Note: 1 kg biogenic carbon is equivalent to 44/12 kg CO2
9 / 11
Additional requirements
Greenhouse gas emissions from the use of electricity in the manufacturing phase
National production mix from import, low voltage (production of transmission lines, in addition to direct emissions and losses in grid) of applied
electricity for the manufacturing process (A3).
Electricity mix Source Amount Unit
Electricity, Norway (kWh) ecoinvent 3.6 24,33 g CO2-eq/kWh
Dangerous substances
The product contains no substances given by the REACH Candidate list.
Indoor environment
Not relevant.
Additional Environmental Information
Additional environmental impact indicators required in NPCR Part A for construction products
Indicator Unit A1-A3 A4 A5 C1 C2 C3 C4 D
GWPIOBC kg CO2 -eq 2,38E-01 5,03E-02 0 0,00E+00 1,42E-02 1,51E+00 7,39E-02 -8,69E-02
GWP-IOBC: Global warming potential calculated according to the principle of instantaneous oxidation. In order to increase the transparency of biogenic carbon​
contribution to climate impact, the indicator GWP-IOBC is required as it declares climate impacts calculated according to the principle of instantaneous oxidation.​
GWP-IOBC is also referred to as GWP-GHG in context to Swedish public procurement legislation.
10 / 11
Bibliography
ISO 14025:2010. Environmental labels and declarations - Type III environmental declarations - Principles and procedures. International
Organization for Standardization.
ISO 14044:2006. Environmental management - Life cycle assessment - Requirements and guidelines. International Organization for
Standardization.
EN 15804:2012+A2:2019. Environmental product declaration - Core rules for the product category of construction products. European
Committee for Standardization.
ISO 21930:2017. Sustainability in buildings and civil engineering works - Core rules for environmental product declarations of construction
products. International Organization for Standardization.
EN 50693:2019. Product category rules for life cycle assessments of electronic and electrical products and systems. European Committee for
Standardization.
Ecoinvent v3, 2019. Allocation, cut-off by classification. Swiss Centre of Life Cycle Inventories.
Iversen et al., (2021). eEPD v2021.09, background information for EPD generator tool system verification, LCA.no. Report number: 07.21. System
verification report.
Philis et al., (2022). EPD generator for NPCR 028 part B for cable pipes, background information for EPD generator application and LCA data,
LCA.no Report number: 06.22. PCR verification report.
EPD Norway (2022). NPCR Part A: Construction products and services. The Norwegian EPD foundation. Version 2.0 published 24.03.2021.
EPD Norway (2022). NPCR 027 Part B for cable pipes. The Norwegian EPD foundation. Version 2.0 published 31.03.2022.
Program operator and publisher Phone: +47 977 22 020
The Norwegian EPD Foundation e-mail: post@epd-norge.no
Post Box 5250 Majorstuen, 0303 Oslo, Norway web: www.epd-norge.no
Owner of the declaration: Phone: +47 32 09 55 99
Hallingplast AS e-mail: post@hallingplast.no
Kleivi næringspark 4, 3570 Ål web: https://www.hallingplast.no/
Author of the Life Cycle Assessment Phone: +47 916 50 916
LCA.no AS e-mail: post@lca.no
Dokka 6A, 1671 Kråkerøy web: www.lca.no
Developer of EPD generator Phone: +47 916 50 916
LCA.no AS e-mail: post@lca.no
Dokka 6A, 1671 Kråkerøy web: www.lca.no
ECO Platform web: www.eco-platform.org
ECO Portal web: ECO Portal
11 / 11
