ENVIRONMENTAL PRODUCT DECLARATION
as per ISO 14025 and EN 15804+A1
Owner of the Declaration ArcelorMittal Construction
Programme holder Institut Bauen und Umwelt e.V. (IBU)
Publisher Institut Bauen und Umwelt e.V. (IBU)
Declaration number EPD-AMC-20210131-CBB1-EN
Issue date 19.01.2022
Valid to 18.01.2027
COFRADAL® 200
ArcelorMittal Construction
www.ibu-epd.com | https://epd-online.com
Umwelt Produktdeklaration Name des Herstellers – Name des Produkts
General Information
ArcelorMittal Construction Cofradal® 200
Programme holder Owner of the declaration
IBU – Institut Bauen und Umwelt e.V. ArcelorMittal Construction
Panoramastr. 1 Morinval
10178 Berlin 55800 Contrisson
Germany France
Declaration number Declared product / declared unit
EPD-AMC-20210131-CBB1-EN The declaration applies to 1m2 of Cofradal® 200.
This declaration is based on the product Scope:
category rules: The Life Cycle Assessment is based on data collected
System floors, 12.2018 from the ArcelorMittal Construction plant in Contrisson
(PCR checked and approved by the SVR) and Montataire in France producing Cofradal 200,
representing 100 % of the annual production from
2018.
Issue date
19.01.2022
The owner of the declaration shall be liable for the
underlying information and evidence; the IBU shall not
Valid to
be liable with respect to manufacturer information, life
18.01.2027
cycle assessment data and evidences.
The EPD was created according to the specifications
of EN 15804+A1. In the following, the standard will be
simplified as EN 15804.
Verification
The standard EN 15804 serves as the core PCR
Independent verification of the declaration and data
according to ISO 14025:2010
Dipl. Ing. Hans Peters internally x externally
(chairman of Institut Bauen und Umwelt e.V.)
Dr. Alexander Röder Mr Carl-Otto Neven
(Managing Director Institut Bauen und Umwelt e.V.)) (Independent verifier)
Product
Product description/Product definition Application
This Environmental Product Declaration refers to Cofradal® 200 is an integrated composite floor system
Cofradal® 200 produced on ArcelorMittal Construction for all types of construction. Its lightness and structural
plants in Contrisson and Montataire. performance allow it to cross large spans (up to 7 m).
Cofradal® 200 is a prefabricated composite floor Despite its low self-weight, Cofradal® floor meets the
system. It includes a specific steel profile, an acoustic requirements of acoustic regulations without the added
and thermal insulation material, as well as a welded ceiling. The 125mm of rock wool Cofradal® allows a
mesh and a concrete slab. fire resistance of REI (min) 120. With an additional
insulation, the needed thermal insulation is reached
For the placing on the market of the product in the with a U value down to 0.20 W/(m2K).
European Union/European Free Trade Association
(EU/EFTA) (with the exception of Switzerland) Technical Data
Regulation (EU) No. 305/2011 (CPR) applies. The technical performance of the product are
essentially covered by EN 1090-1. The steel sheet is a
The product needs a declaration of performance taking S 350 GD grade with metallic coating according to EN
into consideration EN 1090-1, Execution of steel and 10346.
aluminium structures – Part 1: Procedures for
attestation of conformity for load-bearing components, Technical data
and the CE-marking. Name Value Unit
Grammage / system weight 236.6 kg/m2
For the application and use the respective national Sound absorption coefficient (EN
85 %
provisions apply. ISO 354, EN ISO 11654)
Airborne sound reduction (EN
58 dB
20140-9, ISO 140-3)
2 Environmental Product Declaration ArcelorMittal – Cofradal® 200
Compressive strength 30 N/mm² The concrete considered is a C30/37 made out of CEM
Thermal Transmittance (U-Value) 0.78 W/(m².K) I cement, water and aggregates and, when necessary,
additives such as condensers, retarding agents or air-
entraining agents.
Performance data of the product in accordance with
the declaration of performance with respect to its Steel is mainly iron and carbon, with small amounts of
essential characteristics according to EN 1090-1:2009 alloying elements. These elements modify the
Execution of steel and aluminium structures – Part 1: chemical and physical properties of steel such as
Procedures for attestation of conformity for load- strength, durability and corrosion resistance. High
bearing components. strength low alloyed (HSLA) carbon steel has a carbon
content lower than 0.2 %.
Voluntary data: Avis Technique N°3-1/11-687_V2,
Cofradal. This product contains substances listed in the
candidate list (date: 26.2.2020) exceeding 0.1
Base materials/Ancillary materials percentage by mass: no
The product covered by this Environmental Product
Declaration is a Cofradal® 200 ready-to-pour. It is Reference service life
mainly composed of a galvanized steel sheet, rock As a structural part of the building, the Cofradal® 200
wool insulation, steel reinforcements and finally is expected and specified to reach the same service
concrete poured in place. Its finished mass per unit life as that of the building. Considering the main
area is 23.00 kg/m² without concrete and packaging, materials, steel and concrete, the reference service life
and 236.6 kg/m² with poured concrete (after can be up to 100 years.
installation).
LCA: Calculation rules
Declared Unit Module A4 addresses the transportation of Cofradal®
This Environmental Product Declaration 200 to the construction site. Module A5 describes the
represents Cofradal® 200, a prefabricated composite installation of Cofradal® 200 into the building including
floor system. the addition of the welded mesh and concrete.
The declared unit is 1 m², and the EPD refers to a As an integrated system for structural floors, the
manufacturer declaration of type 1b) declaration of one Cofradal® 200 is located in the building internal part
specific product calculated as the mean of products that protects it from bad climatic conditions. It could
produced in several plants of one manufacturer. potentially be also covered by finishing components.
Its use (Module B) within a building does not involve
Declared unit any specific maintenance.
Name Value Unit
Declared unit 1 m2 Within this EPD the modules C1-C4 are included.
conversion factor [Mass/Declared These modules consider the dismantling of the
236.6 -
Unit] to 1 Kg considered product (C1), the transportation of the
This conversion is valid for the final product with its dismantled components (steel, concrete, mineral wool)
concrete installed. to their final EoL destination, the waste processing for
reuse, recovery or recycling (C3) as well as the
disposal (C4)
System boundary
Type of the EPD: cradle-to-gate - with options. Module Comparability
A, B, C and D were considered. Basically, a comparison or an evaluation of EPD data
is only possible if all the data sets to be compared
The following processes were considered in detail for were created according to EN 15804 and the building
the production stages A1-A3: context, respectively the product-specific
 Production of raw materials, production characteristics of performance, are taken into account.
materials (Module A1) and auxiliary materials
(Module A3)
 Transport of raw materials, semi-finished
products and auxiliary materials to the
production site (Module A2)
 Production of steel onsite, including the
production of auxiliary materials on-site,
disposal of production residues and
packaging of raw materials, also taking into
account on-site emissions (Module A3)
 Scrap occurring during the production on-site
is looped back to satisfy some of the demand
for scrap input to the process.
3 Environmental Product Declaration ArcelorMittal – Cofradal® 200
LCA: Scenarios and additional technical information
Transport from the gate to the site (A4)
Name Value Unit
Transport distance 498 km
Capacity utilisation (including
30 %
empty runs)
Assembly (A5)
Name Value Unit
Auxiliary 44 kg
Electricity consumption 10 kWh
Other energy carriers (diesel) 36 MJ
Material loss (steel) 0.3 %
Material loss (concrete) 1 %
End of life (C1-C4)
Name Value Unit
Recycling Steel 85 %
Recycling Concrete 67 %
Energy recovery Mineral Wool 47 %
Landfilling Steel 15 %
Landfilling Concrete 33 %
Landfilling Mineral Wool 53 %
Reuse, recovery and/or recycling potentials (D),
relevant scenario information
Name Value Unit
Recycling Steel 85 %
Recycling Concrete 67 %
Energy Recovery Mineral Wool 47 %
4 Environmental Product Declaration ArcelorMittal – Cofradal® 200
LCA: Results
DESCRIPTION OF THE SYSTEM BOUNDARY (X = INCLUDED IN LCA; MND = MODULE NOT DECLARED;
MNR = MODULE NOT RELEVANT)
BENEFITS AND
CONSTRUCTI LOADS
PRODUCT STAGE ON PROCESS USE STAGE END OF LIFE STAGE BEYOND THE
STAGE SYSTEM
BOUNDARIES
5 Environmental Product Declaration ArcelorMittal – Cofradal® 200
lairetam
waR
ylppus tropsnarT
gnirutcafunaM
eht
morf
tropsnarT
etis
eht
ot
etag
ylbmessA esU
ecnanetniaM
riapeR
tnemecalpeR tnemhsibrufeR
ygrene
lanoitarepO esu
retaw
lanoitarepO esu
noitcurtsnoc-eD
noitilomed tropsnarT
gnissecorp
etsaW
lasopsiD -esueR -yrevoceR -gnilcyceR laitnetop
A1 A2 A3 A4 A5 B1 B2 B3 B4 B5 B6 B7 C1 C2 C3 C4 D
X X X X X X X X X X X X X X X X X
RESULTS OF THE LCA - ENVIRONMENTAL IMPACT according to EN 15804+A1: 1 m² Cofadral® 200
Parameter Unit A1-A3 A4 A5 B1 B2 B3 B4 B5 B6 B7 C1 C2 C3 C4 D
-
4.51E+ 3.10E+ 0.00E+ 0.00E+ 0.00E+ 0.00E+ 0.00E+ 0.00E+ 0.00E+ 2.44E+ 1.41E+ 1.06E+
GWP [kg CO2-Eq.]
1
6.34E-1
1 0 0 0 0 0 0 0 0 0
2.39E-3
0
1.15E+
1
1.49E- 1.27E- 1.07E- 0.00E+ 0.00E+ 0.00E+ 0.00E+ 0.00E+ 0.00E+ 0.00E+ 1.27E- 2.83E- 2.57E- 6.15E- -5.56E-
ODP [kg CFC11-Eq.]
13 16 13 0 0 0 0 0 0 0 13 16 17 15 15
0.00E+ 0.00E+ 0.00E+ 0.00E+ 0.00E+ 0.00E+ 0.00E+ -2.51E-
AP [kg SO2-Eq.] 1.01E-16.96E-44.18E-2
0 0 0 0 0 0 0
1.21E-23.55E-33.43E-66.30E-3
2
0.00E+ 0.00E+ 0.00E+ 0.00E+ 0.00E+ 0.00E+ 0.00E+ -2.49E-
EP [kg (PO4)3--Eq.] 9.51E-31.38E-45.26E-3
0 0 0 0 0 0 0
1.92E-38.33E-47.76E-77.12E-4
3
-1.61E- 0.00E+ 0.00E+ 0.00E+ 0.00E+ 0.00E+ 0.00E+ 0.00E+ -1.10E- -2.99E-
POCP [kg ethene-Eq.] 1.44E-2 4.90E-3 1.23E-3 3.24E-74.88E-4
5 0 0 0 0 0 0 0 3 3
-2.25E- 0.00E+ 0.00E+ 0.00E+ 0.00E+ 0.00E+ 0.00E+ 0.00E+ 3.33E- -4.13E-
ADPE [kg Sb-Eq.] 5.63E-48.15E-8 3.00E-61.81E-7 1.05E-7
5 0 0 0 0 0 0 0 10 7
-
1.25E+ 8.39E+ 1.47E+ 0.00E+ 0.00E+ 0.00E+ 0.00E+ 0.00E+ 0.00E+ 0.00E+ 1.40E+ 1.87E+ 1.48E+
ADPF [MJ] 1.50E-2 9.51E+
3 0 2 0 0 0 0 0 0 0 2 1 1
1
GWP = Global warming potential; ODP = Depletion potential of the stratospheric ozone layer; AP = Acidification potential of land and water; EP =
Caption Eutrophication potential; POCP = Formation potential of tropospheric ozone photochemical oxidants; ADPE = Abiotic depletion potential for non-
fossil resources; ADPF = Abiotic depletion potential for fossil resources
RESULTS OF THE LCA - INDICATORS TO DESCRIBE RESOURCE USE according to EN 15804+A1: 1 m²
Cofadral® 200
Parameter Unit A1-A3 A4 A5 B1 B2 B3 B4 B5 B6 B7 C1 C2 C3 C4 D
PERE [MJ] 5.07E+1 7.04E-1 2.16E+10.00E+00.00E+00.00E+00.00E+00.00E+00.00E+00.00E+04.70E+11.57E+0 6.13E-3 1.94E+0-3.78E+0
PERM [MJ] 0.00E+00.00E+00.00E+00.00E+00.00E+00.00E+00.00E+00.00E+00.00E+00.00E+00.00E+00.00E+00.00E+00.00E+00.00E+0
PERT [MJ] 5.07E+1 7.04E-1 2.16E+10.00E+00.00E+00.00E+00.00E+00.00E+00.00E+00.00E+04.70E+11.57E+0 6.13E-3 1.94E+0-3.78E+0
PENRE [MJ] 1.48E+38.58E+01.57E+20.00E+00.00E+00.00E+00.00E+00.00E+00.00E+00.00E+03.63E+21.91E+1 3.59E-2 1.53E+1-9.70E+1
PENRM [MJ] 0.00E+00.00E+00.00E+00.00E+00.00E+00.00E+00.00E+00.00E+00.00E+00.00E+00.00E+00.00E+00.00E+00.00E+00.00E+0
PENRT [MJ] 1.48E+38.58E+01.57E+20.00E+00.00E+00.00E+00.00E+00.00E+00.00E+00.00E+03.63E+21.91E+1 3.59E-2 1.53E+1-9.70E+1
SM [kg] 5.54E+00.00E+00.00E+00.00E+00.00E+00.00E+00.00E+00.00E+00.00E+00.00E+00.00E+00.00E+00.00E+00.00E+00.00E+0
RSF [MJ] 0.00E+00.00E+00.00E+00.00E+00.00E+00.00E+00.00E+00.00E+00.00E+00.00E+00.00E+00.00E+00.00E+00.00E+00.00E+0
NRSF [MJ] 0.00E+00.00E+00.00E+00.00E+00.00E+00.00E+00.00E+00.00E+00.00E+00.00E+00.00E+00.00E+00.00E+00.00E+00.00E+0
FW [m³] 1.26E-1 9.96E-4 3.14E-2 0.00E+00.00E+00.00E+00.00E+00.00E+00.00E+00.00E+0 1.09E-1 2.22E-3 8.14E-5 3.87E-3-2.10E-2
PERE = Use of renewable primary energy excluding renewable primary energy resources used as raw materials; PERM = Use of
renewable primary energy resources used as raw materials; PERT = Total use of renewable primary energy resources; PENRE = Use of
non-renewable primary energy excluding non-renewable primary energy resources used as raw materials; PENRM = Use of non-
Caption
renewable primary energy resources used as raw materials; PENRT = Total use of non-renewable primary energy resources; SM = Use
of secondary material; RSF = Use of renewable secondary fuels; NRSF = Use of non-renewable secondary fuels; FW = Use of net fresh
water
RESULTS OF THE LCA – WASTE CATEGORIES AND OUTPUT FLOWS according to EN 15804+A1:
1 m² Cofadral® 200
Parameter Unit A1-A3 A4 A5 B1 B2 B3 B4 B5 B6 B7 C1 C2 C3 C4 D
HWD [kg] 6.60E-6 8.42E-7 3.62E-6 0.00E+00.00E+00.00E+00.00E+00.00E+00.00E+00.00E+0 1.21E-5 1.87E-61.39E-102.62E-7-2.45E-7
NHWD [kg] 1.24E+0 9.63E-4 7.37E+00.00E+00.00E+00.00E+00.00E+00.00E+00.00E+00.00E+0 7.63E-2 2.14E-3 3.62E-3 7.13E+1-1.66E-1
RWD [kg] 8.69E-2 4.65E-5 2.74E-3 0.00E+00.00E+00.00E+00.00E+00.00E+00.00E+00.00E+0 8.73E-2 1.04E-4 8.23E-6 2.06E-4-1.34E-4
CRU [kg] 0.00E+00.00E+00.00E+00.00E+00.00E+00.00E+00.00E+00.00E+00.00E+00.00E+00.00E+00.00E+00.00E+00.00E+00.00E+0
MFR [kg] 0.00E+00.00E+00.00E+00.00E+00.00E+00.00E+00.00E+00.00E+00.00E+00.00E+01.46E+20.00E+00.00E+00.00E+00.00E+0
MER [kg] 0.00E+00.00E+00.00E+00.00E+00.00E+00.00E+00.00E+00.00E+00.00E+00.00E+00.00E+00.00E+00.00E+00.00E+00.00E+0
EEE [MJ] 0.00E+00.00E+00.00E+00.00E+00.00E+00.00E+00.00E+00.00E+00.00E+00.00E+00.00E+00.00E+00.00E+00.00E+00.00E+0
EET [MJ] 0.00E+00.00E+00.00E+00.00E+00.00E+00.00E+00.00E+00.00E+00.00E+00.00E+00.00E+00.00E+00.00E+00.00E+00.00E+0
HWD = Hazardous waste disposed; NHWD = Non-hazardous waste disposed; RWD = Radioactive waste disposed; CRU = Components
Caption for re-use; MFR = Materials for recycling; MER = Materials for energy recovery; EEE = Exported electrical energy; EET = Exported
thermal energy
Note: 5,54 kg steel scrap is used in the production/manufacturing of 1 m² of Cofradal® 200. After use, 10,51 kg
steel is recycled. The potential environmental impact calculated for the end-of-life stage (module D) is based on
the net amount of scrap left in the system, which is 10,51 kg – 5,54 kg = 4,97 kg. The system has a net output of
4,97 kg scrap (which carries a potential credit), thus module D shows an environmental benefit.
References
EN 1090-1 General Instructions for the EPD programme of Institut
EN 1090-1:2009+A1:2011, Execution of steel Bauen und Umwelt e.V. Version 2.0, Berlin:
structures and aluminium structures - Part 1: Institut Bauen und Umwelt e.V., 2021. www.ibu-
Requirements for conformity assessment of structural epd.com
components.
PCR Part A
EN 10346 PCR - Part A: Calculation Rules for the Life Cycle
EN 10364:2015, Continuously hot-dip coated steel flat Assessment and Requirements on the Project Report,
products for cold forming - Technical delivery Institut Bauen und Umwelt e.V., www.bauumwelt.com,
conditions. 2019.
EN 15804 PCR Part B
EN 15804:2012-04+A1 2013, Sustainability of PCR - Part B: Requirements on the EPD for System
construction works — Environmental Product floors Version 1.3, Institut Bauen und Umwelt e.V.,
Declarations — Core rules for the product category of www.bauumwelt.com, 2019.
construction products.
Candidate list
ISO 14025 Regulation (EC) No 1907/2006 of the European
DIN EN ISO 14025:2011-10, Environmental labels and Parliament and of the Council on the Registration,
declarations — Type III environmental declarations — Evaluation, Authorisation and Restriction
Principles and procedures. of Chemicals (REACH)
https://echa.europa.eu/candidate-list-table
ISO 14044
DIN EN ISO 14044:2006-10 Environmental Avis Technique N°3-1/11-687_V2
management - Life cycle assessment - Requirements Steel-concrete composite floor slabs – Cofradal.
and guidelines. 13/06/2019. Centre Scientifique et Technique du
Bâtiment. www.cstb.fr
European Commission Technical Steel Research
Sansom, M.and Meijer, J.:Life-cycle assessment (LCA) CPR
for steel construction, European Commission technical Regulation (EU) No 305/2011 of the European
steel research, 2001-12. parliament and of the council of 9 March 2011 laying
down harmonised conditions for the marketing of
GaBi ts Software / Documentation construction products and repealing Council Directive
GaBi ts dataset documentation for the GaBi Software 89/106/EEC.
System and Database for Life Cycle Engineering,
thinkstep AG, Leinfelden-Echterdingen, 2020
(http://documentation.gabi-software.com/)
IBU 2021
6 Environmental Product Declaration ArcelorMittal – Cofradal® 200
Publisher
Institut Bauen und Umwelt e.V. Tel +49 (0)30 3087748- 0
Panoramastr. 1 Fax +49 (0)30 3087748- 29
10178 Berlin Mail info@ibu-epd.com
Germany Web www.ibu-epd.com
Programme holder
Institut Bauen und Umwelt e.V. Tel +49 (0)30 - 3087748- 0
Panoramastr 1 Fax +49 (0)30 – 3087748 - 29
10178 Berlin Mail info@ibu-epd.com
Germany Web www.ibu-epd.com
Author of the Life Cycle
Assessment Tel +49 711 341817-0
Sphera Solutions GmbH Fax +49 711 341817-25
Hauptstraße 111- 113 Mail info@sphera.com
70771 Leinfelden-Echterdingen Web www.sphera.com
Germany
Owner of the Declaration
ArcelorMittal Construction Tel +33 3 29 70 75 03
Morinval - Fax -
55800 Contrisson Mail
France sustainability.amc@arcelormittal.
com
Web construction.arcelormittal.com
