ENVIRONMENTAL PRODUCT DECLARATION
as per ISO 14025 and EN 15804+A2
Owner of the Declaration dormakaba International Holding GmbH
Publisher Institut Bauen und Umwelt e.V. (IBU)
Programme holder Institut Bauen und Umwelt e.V. (IBU)
Declaration number EPD-DOR-20230451-CBA2-EN
Issue date 27.11.2023
Valid to 26.11.2028
Crane Manual Revolving Door - SS 2000/3000
dormakaba
www.ibu-epd.com | https://epd-online.com
General Information
dormakaba Crane Manual Revolving Door - SS 2000/3000
Programme holder Owner of the declaration
IBU – Institut Bauen und Umwelt e.V. dormakaba International Holding GmbH
Hegelplatz 1 DORMA Platz 1
10117 Berlin 58256 Ennepetal
Germany Germany
Declaration number Declared product / declared unit
EPD-DOR-20230451-CBA2-EN 1 piece of the product: Crane Manual Revolving Doors SS 2000/3000, with
a diameter of 7 ft. (2130 mm) and a height of 7,5 ft. (2290 mm), consisting
of the following items:
• 4 door leaves
• Enclosure
• Canopy
• Product packaging
This declaration is based on the product category rules: Scope:
Automatic doors, automatic gates, and revolving door systems, This Environmental Product Declaration refers to a specific manual
01.08.2021 revolving door manufactured by dormakaba. The production site is located
(PCR checked and approved by the SVR) in Reamstown (USA).
The data represents the year 2022.
Issue date The owner of the declaration shall be liable for the underlying information
and evidence; the IBU shall not be liable with respect to manufacturer
27.11.2023
information, life cycle assessment data and evidences.
The EPD was created according to the specifications of EN 15804+A2. In
Valid to
the following, the standard will be simplified as EN 15804.
26.11.2028
Verification
The standard EN 15804 serves as the core PCR
Independent verification of the declaration and data according to ISO
14025:2011
internally X externally
Dipl.-Ing. Hans Peters
(Chairman of Institut Bauen und Umwelt e.V.)
Florian Pronold Matthias Klingler,
(Managing Director Institut Bauen und Umwelt e.V.) (Independent verifier)
1 Environmental Product Declaration - dormakaba - Crane Manual Revolving Door - SS 2000/3000
Product
Product description/Product definition Base materials/Ancillary materials
The Crane Manual Revolving Doors SS 2000/3000 allow both The major material composition including the packaging of the
greater traffic volume and quicker traffic flow. Crane manual product is listed below:
doors are customizable revolving doors. They enable a Name Value Unit
continuous flow of traffic, especially in entrance areas, and at
Stainless Steel 41 %
the same time block the ingress of air. A wide selection of
Glass 37 %
finishes is available to meet projects needs.
Steel 10 %
For the Crane Manual Revolving Doors SS 2000/3000 the Zinc 6 %
standards which can be applied are the following: Plastics 3 %
• ANSI 156.27 Paper 2 %
Aluminium 1 %
Application The product includes partial articles which contain substances
Revolving doors may be used to provide a comfortable entry listed in the Candidate List of REACH Regulation
and exit in many applications in the facade of or within a 1907/2006/EC (date: 14.06.2023) exceeding 0.1 percentage by
building. Typical applications include: mass: no
• Hotels
The Candidate List can be found on the ECHA website
• Healthcare settings
address: https:echa.europa.eu/de/home.
• Airports and transportation facilities
• Commercial office buildings Reference service life
• Institutional and educational buildings
The reference service life of the Manual Revolving Door SS
• Retail stores
2000/3000 amounts to 30 years, depending on the application
and frequency of use. For repairs and renewals, suitable spare
Technical Data
parts are available. The revolving door is tested and certified to
The Crane manual revolving doors SS 2000/3000 have
ANSI 156.27, meaning they are designed to withstand a
following technical properties:
minimum of 1.000.000 cycles.
Name Value Unit
Height range 1000/2000 7-9 ft
Height range 3000 7+ ft
Diameter range maximum
12 ft
1000/2000/3000
clear or tinted
Enclosure glass 1000/2000 7/16"
laminated
clear or tinted
Enclosure glass 3000 9/16"
laminated
Door leaf glass 1/4" tempered
The product with respect to its characteristics is in accordance
with the relevant technical provisions (no CE-marking):
• ANSI 156.27
LCA: Calculation rules
Production - Module A1-A3
Declared Unit The product stage includes:
— A1, raw material extraction, processing and mechanical
The declared unit is 1 piece of the product: Manual Revolving treatments, processing of secondary material input (e.g.
Door SS 2000/3000 including packaging recycling processes),
Name Value Unit — A2, transport to the manufacturer,
— A3, manufacturing and assembly including provision of all
Declared unit 1 piece/product
materials, products and energy, as well as waste processing up
Mass of declared Product 684 kg
to the end-of-waste state.
Construction stage - Modules A4-A5
System boundary
The construction process stage includes:
The type of EPD is: cradle to gate with options, modules C1– — A4, transport to the building site;
C4, and module D (A1–A3 + C + D and additional modules: — A5, installation into the building;
A4+ A5) including provision of all materials, products and energy, as well
as waste processing up to the end-of-waste state or disposal of
final residues during the construction process stage.
2 Environmental Product Declaration - dormakaba - Crane Manual Revolving Door - SS 2000/3000
End-of-life stage– Modules C1-C4 and D
The end-of-life stage includes: Geographic Representativeness
— C1, de-construction, demolition: Land or region, in which the declared product system is
— C2, transport to waste processing; manufactured, used or handled at the end of the product´s
— C3, waste processing for reuse, recovery and/or recycling; lifespan: Global
— C4, disposal;
including provision and all transport, provision of allmaterials,
Comparability
products and related energy and water use.
Basically, a comparison or an evaluation of EPD data is only
possible if all the data sets to be compared were created
Module D (Benefits and loads beyond the system boundary)
according to EN 15804 and the building context, respectively
includes:
the product-specific characteristics of performance, are taken
— D, recycling potentials, expressed as net impacts and
into account. Background database: GaBi, SP40.
benefits.
LCA: Scenarios and additional technical information
End of life (C1-C4)
Characteristic product properties of biogenic carbon
C1: The product expansion depends on the building. The
Information on describing the biogenic carbon content at product share is so low that no environmental burden is
factory gate assumed.
Name Value Unit C2: Transport to waste management is 50 km.
Biogenic carbon content in product 4.18 kg C Name Value Unit
Note: 1 kg of biogenic carbon is equivalent to 44/12 kg of CO . Collected separately waste type waste type 675 kg
2
Recycling 408 kg
Energy recovery 14.2 kg
Landfilling 252 kg
Transport to the building site (A4)
The product is disassembled in a recycling process. Material
Name Value Unit recycling is then assumed for the metals and electronics. The
Litres of fuel 0.00276 l/100km plastic components are assumed to be incinerated with energy
recovery. Minor proportions of residues arising from the
Transport distance 50 km
recycling process are landfilled. Region for the End of Life is:
Capacity utilisation (including empty runs) 55 %
Global.
The product is transported via truck. The main distribution
region is North America. In order to allow scaling to a specific
Reuse, recovery and/or recycling potentials (D), relevant
point of installation 100 km are declared.
scenario information
Name Value Unit
Installation into the building (A5)
Recycling 100 %
Name Value Unit
The collection rate is 100 %.
Waste packaging (paper and plastic) 9 kg
Reference service life
Name Value Unit
Life Span according to the manufacturer 30 a
3 Environmental Product Declaration - dormakaba - Crane Manual Revolving Door - SS 2000/3000
LCA: Results
DESCRIPTION OF THE SYSTEM BOUNDARY (X = INCLUDED IN LCA; MND = MODULE OR INDICATOR NOT DECLARED; MNR
= MODULE NOT RELEVANT)
Benefits and
Construction loads beyond
Product stage Use stage End of life stage
process stage the system
boundaries
la ire ta m w a Ry lp p u s tro p s n a rT g n iru tc a fu n a M e h t m o rf tro p s n a rTe tis e h t o t e ta g y lb m e s s A e s U e c n a n e tn ia M ria p e R tn e m e c a lp e R tn e m h s ib ru fe R y g re n e la n o ita re p Oe s u re ta w la n o ita re p Oe s u n o itc u rts n o c -e Dn o itilo m e d tro p s n a rT g n is s e c o rp e ts a W la s o p s iD -e s u e R-y re v o c e R-g n ilc y c e Rla itn e to p
A1 A2 A3 A4 A5 B1 B2 B3 B4 B5 B6 B7 C1 C2 C3 C4 D
X X X X X MND MND MNR MNR MNR MND MND X X X X X
RESULTS OF THE LCA - ENVIRONMENTAL IMPACT according to EN 15804+A2: 1 piece Crane SS 2000/3000
Parameter Unit A1-A3 A4 A5 C1 C2 C3 C4 D
GWP-total kg CO 2 eq 3.19E+03 5.98E+00 2.29E+01 0 2.95E+00 6.12E+01 3.85E+00 -1.55E+03
GWP-fossil kg CO 2 eq 3.21E+03 5.72E+00 2.29E+01 0 2.82E+00 4.09E+01 3.83E+00 -1.55E+03
GWP-biogenic kg CO 2 eq -2.07E+01 2.64E-01 5.33E-04 0 1.3E-01 2.03E+01 1.3E-02 5.7E+00
GWP-luluc kg CO 2 eq 4.05E+00 1.36E-04 1E-03 0 6.71E-05 2E-03 1.1E-02 -2.58E+00
ODP kg CFC11 eq 1.4E-10 6.03E-16 1.15E-14 0 2.98E-16 2.3E-14 1.42E-14 -3.61E-10
AP mol H+ eq 1.48E+01 6E-03 4E-03 0 3E-03 1E-02 2.7E-02 -6.67E+00
EP-freshwater kg P eq 3.55E-03 1.22E-06 1.84E-06 0 6.04E-07 3.64E-06 6.57E-06 -2E-03
EP-marine kg N eq 2.39E+00 2E-03 9.18E-04 0 8.98E-04 3E-03 7E-03 -1.04E+00
EP-terrestrial mol N eq 2.63E+01 2E-02 1.9E-02 0 1E-02 4.7E-02 7.8E-02 -1.12E+01
kg NMVOC
POCP 6.46E+00 5E-03 3E-03 0 3E-03 7E-03 2.1E-02 -3.17E+00
eq
ADPE kg Sb eq 2.1E-01 1.71E-07 1.58E-07 0 8.46E-08 3.21E-07 3.44E-07 -9.3E-02
ADPF MJ 4.49E+04 8.1E+01 1.06E+01 0 4E+01 2.32E+01 5.02E+01 -1.88E+04
m3 world eq
WDP 9.23E+02 1.1E-02 2.34E+00 0 6E-03 6.28E+00 4.01E-01 -5.54E+02
deprived
GWP = Global warming potential; ODP = Depletion potential of the stratospheric ozone layer; AP = Acidification potential of land and water; EP =
Eutrophication potential; POCP = Formation potential of tropospheric ozone photochemical oxidants; ADPE = Abiotic depletion potential for non-fossil
resources; ADPF = Abiotic depletion potential for fossil resources; WDP = Water (user) deprivation potential)
RESULTS OF THE LCA - INDICATORS TO DESCRIBE RESOURCE USE according to EN 15804+A2: 1 piece Crane SS
2000/3000
Parameter Unit A1-A3 A4 A5 C1 C2 C3 C4 D
PERE MJ 8.96E+03 2.56E-01 2.76E+00 0 1.26E-01 1.42E+02 6.58E+00 -3.9E+03
PERM MJ 1.36E+02 0 0 0 0 -1.36E+02 0 0
PERT MJ 9.09E+03 2.56E-01 2.76E+00 0 1.26E-01 5.72E+00 6.58E+00 -3.9E+03
PENRE MJ 4.41E+04 8.11E+01 3.98E+02 0 4E+01 5.33E+02 5.02E+01 -1.89E+04
PENRM MJ 8.96E+02 0 -3.87E+02 0 0 -5.09E+02 0 0
PENRT MJ 4.5E+04 8.11E+01 1.06E+01 0 4E+01 2.32E+01 5.02E+01 -1.89E+04
SM kg 1.32E+02 0 0 0 0 0 0 0
RSF MJ 0 0 0 0 0 0 0 0
NRSF MJ 0 0 0 0 0 0 0 0
FW m3 3.33E+01 4.58E-04 5.6E-02 0 2.26E-04 1.49E-01 1.3E-02 -2.19E+01
PERE = Use of renewable primary energy excluding renewable primary energy resources used as raw materials; PERM = Use of renewable primary
energy resources used as raw materials; PERT = Total use of renewable primary energy resources; PENRE = Use of non-renewable primary energy
excluding non-renewable primary energy resources used as raw materials; PENRM = Use of non-renewable primary energy resources used as raw
materials; PENRT = Total use of non-renewable primary energy resources; SM = Use of secondary material; RSF = Use of renewable secondary fuels;
NRSF = Use of non-renewable secondary fuels; FW = Use of net fresh water
RESULTS OF THE LCA – WASTE CATEGORIES AND OUTPUT FLOWS according to EN 15804+A2:
1 piece Crane SS 2000/3000
Parameter Unit A1-A3 A4 A5 C1 C2 C3 C4 D
HWD kg 1.41E-04 7.87E-09 4.04E-08 0 3.88E-09 7.48E-08 7.65E-07 -1.74E-04
NHWD kg 2.52E+02 8E-03 2.38E+00 0 4E-03 4.36E+00 2.52E+02 -1.2E+02
RWD kg 1.81E+00 8.71E-05 3.94E-04 0 4.3E-05 9.51E-04 5.72E-04 -2.62E-01
CRU kg 0 0 0 0 0 0 0 0
MFR kg 0 0 0 0 0 3.95E+02 0 0
MER kg 0 0 0 0 0 0 0 0
EEE MJ 0 0 4.24E+01 0 0 1.05E+02 0 0
EET MJ 0 0 9.73E+01 0 0 2.26E+02 0 0
4 Environmental Product Declaration - dormakaba - Crane Manual Revolving Door - SS 2000/3000
HWD = Hazardous waste disposed; NHWD = Non-hazardous waste disposed; RWD = Radioactive waste disposed; CRU = Components for re-use;
MFR = Materials for recycling; MER = Materials for energy recovery; EEE = Exported electrical energy; EET = Exported thermal energy
RESULTS OF THE LCA – additional impact categories according to EN 15804+A2-optional:
1 piece Crane SS 2000/3000
Parameter Unit A1-A3 A4 A5 C1 C2 C3 C4 D
Disease
PM 2E-04 3.01E-08 5.2E-08 0 1.48E-08 1.07E-07 3.4E-07 -1.28E-04
incidence
IR kBq U235 eq 1.72E+02 1.2E-02 3.5E-02 0 6E-03 1.03E-01 5.9E-02 -3.65E+01
ETP-fw CTUe 2.51E+04 5.74E+01 3.98E+00 0 2.83E+01 8.99E+00 2.87E+01 -9.17E+03
HTP-c CTUh 4.02E-04 1.08E-09 3.45E-10 0 5.33E-10 7.39E-10 4.25E-09 -2.1E-06
HTP-nc CTUh 5.82E-05 4.62E-08 3.49E-08 0 2.28E-08 6.63E-08 4.68E-07 5.1E-05
SQP SQP 8.28E+03 2.08E-01 3.18E+00 0 1.03E-01 6.86E+00 1.05E+01 -2.38E+03
PM = Potential incidence of disease due to PM emissions; IR = Potential Human exposure efficiency relative to U235; ETP-fw = Potential comparative
Toxic Unit for ecosystems; HTP-c = Potential comparative Toxic Unit for humans (cancerogenic); HTP-nc = Potential comparative Toxic Unit for humans
(not cancerogenic); SQP = Potential soil quality index
Disclaimer 1 – for the indicator “Potential Human exposure efficiency relative to U235”. This impact category deals mainly with the
eventual impact of low-dose ionizing radiation on human health of the nuclear fuel cycle. It does not consider effects due to possible
nuclear accidents, occupational exposure or radioactive waste disposal in underground facilities. Potential ionizing radiation from the
soil, radon and from some construction materials is also not measured by this indicator.
Disclaimer 2 – for the indicators “abiotic depletion potential for non-fossil resources”, “abiotic depletion potential for fossil resources”,
“water (user) deprivation potential, deprivation-weighted water consumption”, “potential comparative toxic unit for ecosystems”,
“potential comparative toxic unit for humans – cancerogenic”, “Potential comparative toxic unit for humans - not cancerogenic”,
“potential soil quality index”. The results of this environmental impact indicator shall be used with care as the uncertainties on these
results are high as there is limited experience with the indicator.
This EPD was created using a software tool.
References
ANSI 156.27 GaBi ts documentation
ANSI/BHMA A156.27-2019, Power and Manual Operated GaBi life cycle inventory data documentation
Revolving Pedestrian Doors (https://www.gabisoftware.com/support/gabi/gabidatabase-
2020-lcidocumentation/).
EN 15804
EN 15804+A2:2019+AC:2021, LCA-tool dormakaba
Sustainability of construction works — Environmental Product Tool No.: IBU-DOR-202107-LT1-EN .
Declarations — Core rules for the product category of Developed by Sphera Solutions GmbH
construction products
PCR Part A
ISO 14025 PCR – Part A: Calculation Rules for the Life Cycle Assessment
DIN EN ISO 14025:201110, Environmental labels and and Requirements on the Project Re-port according to EN
declarations — Type III environmental declarations — 15804+A2:2019, Version 1.0, 2020,
Principles and procedures Institut Bauen und Umwelt e.V.,
www.ibu-epd.com.
REACH
Regulation (EC) No 1907/2006 of the European Parliament and PCR Part B PCR – Part B: Requirements on the EPD for
of the Council on the Registration, Evaluation, Authorisation Automatic doors,
and Restriction of Chemicals (REACH) automatic gates, and revolving door systems, Version 6, 2023,
Institut Bauen und Umwelt e.V.,
Further References www.ibu-epd.com.
IBU 2021
General Instructions for the EPD programme of Institut Bauen
und Umwelt e.V. Version 2.0, Berlin: Institut Bauen und Umwelt
e.V., 2021. www.ibu-epd.com
GaBi
Sphera Solutions GmbH
Gabi Software System and Database for Life Cycle Engineering
19922020
Version 10.0.0.71
University of Stuttgart
Leinfelden-Echterdingen
5 Environmental Product Declaration - dormakaba - Crane Manual Revolving Door - SS 2000/3000
Publisher
Institut Bauen und Umwelt e.V. +49 (0)30 3087748- 0
Hegelplatz 1 info@ibu-epd.com
10117 Berlin www.ibu-epd.com
Germany
Programme holder
Institut Bauen und Umwelt e.V. +49 (0)30 3087748- 0
Hegelplatz 1 info@ibu-epd.com
10117 Berlin www.ibu-epd.com
Germany
Author of the Life Cycle Assessment
dormakaba International Holding GmbH +49 2333 793-0
DORMA Platz 1 info.de@dormakaba.com
58256 Ennepetal www.dormakaba.com
Germany
Owner of the Declaration
dormakaba International Holding GmbH +49 2333 793-0
DORMA Platz 1 info.de@dormakaba.com
58256 Ennepetal www.dormakaba.com
Germany
6 Environmental Product Declaration - dormakaba - Crane Manual Revolving Door - SS 2000/3000
