ver1 2015
ENVIRONMENTAL PRODUCT DECLARATION
in accordance with ISO 14025, ISO 21930 and EN 15804
Owner of the declaration: Saint-Gobain Sweden AB, Scanspac
Program operator: The Norwegian EPD Foundation
Publisher: The Norwegian EPD Foundation
Declaration number: NEPD-3479-2078-EN
Registration number: NEPD-3479-2078-EN
ECO Platform reference number: -
Issue date: 29.04.2022
Valid to: 29.04.2027
Dalapro Wood Finish Plus
Saint-Gobain Sweden AB, Scanspac
www.epd-norge.no
NEPD-3479-2078-EN Dalapro Wood Finish Plus
1 / 8
General information
Product: Owner of the declaration:
Dalapro Wood Finish Plus
Saint-Gobain Sweden AB, Scanspac
Contact person: Christian Nilsson
Phone: +46 (0)19-46 34 00
e-mail: ehs.scanspac@dalapro.com
Program operator: Manufacturer:
Saint-Gobain Sweden AB, Scanspac
The Norwegian EPD Foundation
Pb. 5250 Majorstuen, 0303 Oslo
Phone: +47 23 08 80 00
e-mail: post@epd-norge.no
Declaration number: Place of production:
Saint-Gobain Sweden AB, Scanspac
NEPD-3479-2078-EN Kemivägen 7 SE-705 97 Glanshammar
Sweden
ECO Platform reference number: Management system:
ISO 9001, ISO 14001
This declaration is based on Product Category Rules: Organisation no:
556241-2592
CEN Standard EN 15804:2012+A1:2013 serves as core PCR.
NPCR 009:2018 Part B for Technical - Chemical products in the building and
construction industry
Statement of liability: Issue date: 29.04.2022
The owner of the declaration shall be liable for the underlying information and
evidence. EPD Norway shall not be liable with respect to manufacturer Valid to: 29.04.2027
information, life cycle assessment data and evidences.
Declared unit: Year of study:
1 kg Dalapro Wood Finish Plus 2020
Declared unit with option: Comparability:
EPD of construction products may not be comparable if they not comply with EN
A1,A2,A3,A4
15804 and seen in a building context.
Functional unit: Development and verification of EPD:
The declaration has been developed and verified using EPD tool lca.tools
ver EPD2020.11, developed by LCA.no AS. The EPD tool is integrated into
the company's environmental management system, and has been
approved by EPD-Norway
General information on verification of EPD from EPD tools:
Independent verification of data, other environmental information and Developer of EPD:
the declaration according to ISO 14025:2010, § 8.1.3 and § 8.1.4. Individual
third party verification of each EPD is not required when the EPD tool is i) Ellinor Johansson
integrated into the company's environmental management system, ii) the
procedures for use of the EPD tool are approved by EPDNorway, and iii) Reviewer of company-specific input data and EPD:
the proccess is reviewed annualy. See Appendix G of EPD-Norway's
General Programme Instructions for further information on EPD tools. Christian Borgenfalk
Verification of EPD tool: Approved:
Independent third party verification of the EPD tool, background data
Sign
and test-EPD in accordance with EPDNorway's procedures and guidelines
for verification and approval of EPD tools.
Anne Rønning, Norsus AS
(no signature required) Håkon Hauan, CEO EPD-Norge
NEPD-3479-2078-EN Dalapro Wood Finish Plus
2 / 8
Product
Product description: Technical data:
Dalapro Wood Finish Plus is a ready-mixed, extra fine hand filler for TECHNICAL DATA
woodwork. Use the product for filling frames, doors, hatches and suchlike Binding agent: Latex co-polymer
indoors. Good adhesion, strength and building properties make the Solvent: Water
smoothed surface an excellent base coat for woodwork and enamel Grain size: Max. 0.03 mm
paint. White color. Nordic Ecolabelled. pH: Approx. 9
Colour: White
Product specification
Packaging: 200 ml and 400 ml tubes. 3 litre plastic bucket. Market:
Europe
Dalapro Wood Finish Plus 3 litre is packaged in a bucket manufactured in
100 % recyclable plastic and consists Reference service life, product
of at least 90 % recycled plastic.
Filler has a limited shelf life and is date-marked.
Unopened packaging can be kept in a dark place, free
All calculations of the packaging material is made with the 3 litre bucket
from frost, for up to 12 months. Containers that have
that represent the majority of the market.
been opened must be sealed well.
Materials %
Reference service life, building
Filler-dolomite 50-75
Water 10-25 Not included in the declaration
Binder 2,5-10
Additive 1-2,5
Packaging
Pallet
LCA: Calculation rules
Declared unit: Allocation:
The allocation is made in accordance with the provisions of EN 15804.
1 kg Dalapro Wood Finish Plus
Incoming energy and water and waste production in-house is allocated
Cut-off criteria: equally among all products through mass allocation. Effects of primary
production of recycled materials is allocated to the main product in
All major raw materials and all the essential energy is included. The
which the material was used. The recycling process and transportation of
production processes for raw materials and energy flows with very small
the material is allocated to this analysis.
amounts (less than 1%) are not included. These cut-off criteria do not
apply for hazardous materials and substances.
Data quality:
Specific data for the product composition are provided by the manufacturer. They represent the production of the declared product and were collected for
EPD development in the year of study. Background data is based on registered EPDs according to EN 15804, Ostfold Research databases, ecoinvent and other
LCA databases. The data quality of the raw materials in A1 is presented in the table below.
Materials Source Data quality Year
Chemicals Chemicals below cut-off No data 0
Cellulose Ether ecoinvent 3.4 Database 2017
Filler ecoinvent 3.4 Database 2017
Packaging ecoinvent 3.4 Database 2017
Water ecoinvent 3.4 Database 2017
Packaging Modified ecoinvent 3.4 Database 2017
Packaging Supplier Specific 2020
NEPD-3479-2078-EN Dalapro Wood Finish Plus
3 / 8
System boundary:
The flowchart shows the system boundaries A1-A4.
Additional technical information:
The product meets CE-marking requirements in accordance with EN 15824.
NEPD-3479-2078-EN Dalapro Wood Finish Plus
4 / 8
LCA: Scenarios and additional technical information
The following information describe the scenarios in the different modules of the EPD.
Transport from production place to user (A4)
Capacity utilisation Fuel/Energy
Type Type of vehicle Distance km Unit Value (l/t)
(incl. return) % consumption
Truck 55,0 % Truck, lorry over 32 tonnes, EURO 6 300 0,022606 l/tkm 6,78
Railway l/tkm
Boat l/tkm
Other Transportation l/tkm
NEPD-3479-2078-EN Dalapro Wood Finish Plus
5 / 8
LCA: Results
The LCA results are presented below for the declared unit defined on page 2 of the EPD document.
System boundaries (X=included, MND=module not declared, MNR=module not relevant)
Construction Beyond the
Product stage installation User stage End of life stage . system
stage bondaries
A1 A2 A3 A4 A5 B1 B2 B3 B4 B5 B6 B7 C1 C2 C3 C4 . D
X X X X .
Environmental impact
Parameter Unit A1 A2 A3 A4
GWP kg CO 2 -eq 3,21E-01 6,77E-03 9,45E-03 2,48E-02
ODP kg CFC11 -eq 3,28E-08 1,32E-09 8,51E-10 5,10E-09
POCP kg C 2H 4-eq 2,00E-04 1,09E-06 4,55E-06 3,88E-06
AP kg SO 2 -eq 3,21E-03 2,20E-05 6,45E-05 6,41E-05
EP kg PO 3- -eq 6,18E-04 3,69E-06 3,94E-05 8,84E-06
4
ADPM kg Sb -eq 2,40E-06 1,53E-08 2,82E-08 5,91E-08
ADPE MJ 6,03E+00 1,06E-01 5,40E-02 4,08E-01
GWP Global warming potential; ODP Depletion potential of the stratospheric ozone layer; POCP Formation potential of tropospheric photochemical oxidants;
AP Acidification potential of land and water; EP Eutrophication potential; ADPM Abiotic depletion potential for non fossil resources; ADPE Abiotic depletion
potential for fossil resources
Reading example: 9,0 E-03 = 9,0*10-3 = 0,009
*INA Indicator Not Assessed
waR slairetam tropsnarT gnirutcafunaM tropsnarT ylbmessA esU ecnanetniaM riapeR tnemecalpeR tnemhsibrufeR lanoitarepO ygrene esu lanoitarepO esu
retaw
-eD noitcurtsnoc noitilomed tropsnarT etsaW gnissecorp lasopsiD -yrevoceR-esueR -gnilcyceR laitnetop
NEPD-3479-2078-EN Dalapro Wood Finish Plus
6 / 8
Resource use
Parameter Unit A1 A2 A3 A4
RPEE MJ 1,23E+00 1,92E-03 2,88E-01 7,41E-03
RPEM MJ 6,43E-01 0,00E+00 5,36E-04 0,00E+00
TPE MJ 1,88E+00 1,92E-03 2,88E-01 7,41E-03
NRPE MJ 5,62E+00 1,10E-01 9,25E-02 4,20E-01
NRPM MJ 1,41E+00 0,00E+00 0,00E+00 0,00E+00
TRPE MJ 7,03E+00 1,10E-01 9,25E-02 4,20E-01
SM kg 2,38E-02 0,00E+00 0,00E+00 0,00E+00
RSF MJ 0,00E+00 0,00E+00 0,00E+00 0,00E+00
NRSF MJ 0,00E+00 0,00E+00 0,00E+00 0,00E+00
W m3 4,22E-03 2,58E-05 6,69E-04 9,95E-05
RPEE Renewable primary energy resources used as energy carrier; RPEM Renewable primary energy resources used as raw materials; TPE Total use of renewable
primary energy resources; NRPE Non renewable primary energy resources used as energy carrier; NRPM Non renewable primary energy resources used as
materials; TRPE Total use of non renewable primary energy resources; SM Use of secondary materials; RSF Use of renewable secondary fuels; NRSF Use of non
renewable secondary fuels; W Use of net fresh water
Reading example: 9,0 E-03 = 9,0*10-3 = 0,009
*INA Indicator Not Assessed
End of life - Waste
Parameter Unit A1 A2 A3 A4
HW kg 7,31E-06 5,82E-08 3,72E-03 2,24E-07
NHW kg 2,39E-01 9,94E-03 1,25E-02 3,84E-02
RW kg INA* INA* INA* INA*
HW Hazardous waste disposed; NHW Non hazardous waste disposed; RW Radioactive waste disposed
Reading example: 9,0 E-03 = 9,0*10-3 = 0,009
*INA Indicator Not Assessed
End of life - Output flow
Parameter Unit A1 A2 A3 A4
CR kg 0,00E+00 0,00E+00 0,00E+00 0,00E+00
MR kg 0,00E+00 0,00E+00 8,00E-04 0,00E+00
MER kg 0,00E+00 0,00E+00 4,73E-03 0,00E+00
EEE MJ INA* INA* INA* INA*
ETE MJ INA* INA* INA* INA*
CR Components for reuse; MR Materials for recycling; MER Materials for energy recovery; EEE Exported electric energy; ETE Exported thermal energy
Reading example: 9,0 E-03 = 9,0*10-3 = 0,009
*INA Indicator Not Assessed
NEPD-3479-2078-EN Dalapro Wood Finish Plus
7 / 8
Additional Norwegian requirements
Greenhouse gas emissions from the use of electricity in the manufacturing phase
National production mix from import, low voltage (production of transmission lines, in addition to direct emissions and losses in grid) of applied electricity for
the manufacturing process (A3).
Electricity mix Data source Amount Unit
Renewable electricity with Guarantee of Origin from LOS (kWh) Modified ecoinvent 3.4 60,20 g CO2-ekv/kWh
Dangerous substances
The product contains no substances given by the REACH Candidate list or the Norwegian priority list.
Indoor environment
Bibliography
ISO 14025:2010 Environmental labels and declarations - Type III environmental declarations - Principles and procedures.
ISO 14044:2006 Environmental management - Life cycle assessment - Requirements and guidelines.
EN 15804:2012+A1:2013 Environmental product declaration - Core rules for the product category of construction products.
ISO 21930:2017 Sustainability in buildings and civil engineering works. Core rules for environmental product declarations of construction products.
ecoinvent v3, Allocation, cut-off by classification, Swiss Centre of Life Cycle Inventories.
Iversen et al., (2018) eEPD v3.0 - Background information for EPD generator system, LCA.no report number 04.18
Iversen et al., (2019) EPD generator for Saint-Gobain Weber and Scanspac - Background information and LCA data, LCA.no report number 05.18
NPCR Part A: Construction products and services. Ver. 1.0. April 2017, EPD-Norge.
NPCR 009 Part B for technical-chemical products. Ver. 1.0 June 2018, EPD-Norge.
Program operator and publisher Phone: +47 23 08 80 00
The Norwegian EPD Foundation e-mail: post@epd-norge.no
Post Box 5250 Majorstuen, 0303 Oslo,Norway web: www.epd-norge.no
Owner of the declaration Phone: +46 (0)19-46 34 00
Saint-Gobain Sweden AB, Scanspac e-mail: ehs.scanspac@dalapro.com
Kemivägen 7 SE-705 97 Glanshammar web: www.dalapro.se
Author of the Life Cycle Assessment Phone: +47 916 50 916
LCA.no AS e-mail: post@lca.no
Dokka 1C 1671 Kråkerøy web: www.lca.no
Developer of EPD generator Phone: +47 916 50 916
LCA.no AS e-mail: post@lca.no
Dokka 1C,1671 Kråkerøy web: www.lca.no
NEPD-3479-2078-EN Dalapro Wood Finish Plus
8 / 8
