Environmental product declaration
in accordance with ISO 14025 and EN 15804+A2
DBB Air insulated switchgear Type: AH12 - Comprising of Outgoing & Incoming
feeders, Buscoupler & Bus sectionalizer with Transfer
Owner of the declaration: Program operator:
Al-Ahleia Switchgear Co., k.s.c.c The Norwegian EPD Foundation
Product: Declaration number:
DBB Air insulated switchgear Type: AH12 - Comprising of NEPD-8816-8478
Outgoing & Incoming feeders, Buscoupler & Bus
Registration number:
sectionalizer with Transfer
NEPD-8816-8478
Declared unit:
1 pcs
Issue date: 23.01.2025
This declaration is based on Product Category Rules:
Valid to: 23.01.2030
The Norwegian EPD Foundation CEN Standard EN 15804:2012+A2:2019, EN 50693:2019
and PCR EPD Italy 007 serves as core PCR EPD software:
PCR EPDItaly015 - Electronic and electrical products and LCAno EPD generator ID: 626170
systems - Switchboards
1/13
General information
Product Owner of the declaration:
DBB Air insulated switchgear Type: AH12 - Comprising of Outgoing & Al-Ahleia Switchgear Co., k.s.c.c
Incoming feeders, Buscoupler & Bus sectionalizer with Transfer Contact person: Manoj C.G
Phone: +965 24271000
Program operator: e-mail: ahleia@ahleiasg.com
The Norwegian EPD Foundation
Manufacturer:
Post Box 5250 Majorstuen, 0303 Oslo, Norway
Phone: +47 977 22 020 Al-Ahleia Switchgear Co., k.s.c.c
web: www.epd-norge.no
Declaration number:
NEPD-8816-8478
Place of production:
This declaration is based on Product Category Rules:
Al-Ahleia Switchgear Co., k.s.c.c
CEN Standard EN 15804:2012+A2:2019, EN 50693:2019 and PCR EPD
Italy 007 serves as core PCR , Kuwait
PCR EPDItaly015 - Electronic and electrical products and systems -
Switchboards Management system:
ISO 9001, 14001, 29001 and 45001
Statement of liability:
The owner of the declaration shall be liable for the underlying
information and evidence. EPD Norway shall not be liable with
respect to manufacturer information, life cycle assessment data and
evidences. Organisation no:
33118
Declared unit:
1 pcs DBB Air insulated switchgear Type: AH12 - Comprising of
Outgoing ​& Incoming feeders, Buscoupler & Bus sectionalizer with
Transfer
Issue date:
Declared unit with option:
23.01.2025
A1-A3,A4,A5,B1,B6,C1,C2,C3,C4,D
Functional unit:
Valid to:
Functional unit - 1 Set of DBB switchgear units comprising of
23.01.2030
varieties Outgoing feeder, Incomer feeder, Buscoupler and Bus
sectionalizer with Transfer, 1 pc each of Type: AH12, Rating: 12kV,
Year of study:
40kA with a use rate of 99.5% and average load factor of 32%
2023
(assembly of electrical and electronic devices delivering control,
distribution & safety functions) manufactured and installed, used Comparability:
over a life time of 25 years, including waste treatment at end of life.
EPD for electronic and electrical products and systems may not be
comparable if they do not comply with similar PCR standards.
General information on verification of EPD from EPD tools:
Independent verification of data, other environmental information
and the declaration according to EN ISO 14025:2010, § 8.1.3 and §
Development and verification of EPD:
8.1.4. Verification of each EPD is made according to EPD-Norway’s
The declaration is created using EPD tool lca.tools ver EPD2022.03,
guidelines for verification and approval requiring that tools are i)
developed by LCA.no. The EPD tool is integrated in the company's
integrated into the company's environmental management system, ii)
management system, and has been approved by EPD Norway.
the procedures for use of the EPD tool are approved by EPD-Norway,
and iii) the process is reviewed annually by an independent third
Developer of EPD: Zohaib Ali
party verifier. See Appendix G of EPD-Norway's General Programme
Instructions for further information on EPD tools Reviewer of company-specific input data and EPD: Børge Heggen
Johansen, Energiråd AS
Verification of EPD tool:
Independent third party verification of the EPD tool, background data
and test-EPD in accordance with EPDNorway's procedures and
Approved:
guidelines for verification and approval of EPD tools. Approval
number: NEPDT57.
Third party verifier:
Elisabet Amat, GREENIZE projects
(no signature required)
2/13
Product
Product description:
Al-Ahleia make DBB Air insulated switchgear Type: AH12 is an indoor, totally enclosed type metal clad switchgear equipped with a horizontal
isolation Switching Device and two disconnectors, one for each busbar, to enable switchgear service continuity. Type: AH12 Switchgear fulfil the
common need of controlling, protecting and isolating power systems. DBB Type: AH12 Switchgear is designed to offer a very high level of
reliability as the feeder cables can be changed over from one busbar to the other without loss of power. Each of the variety in DBB switchgear is
equipped with integral or withdrawable type earthing switch as applicable.
The DBB switchgear described in this declaration cover varieties like Outgoing feeder, Incomer feeder, Bus coupler, Bus sectionalizer with transfer
unit.
Product specification
Al-Ahleia make DBB switchgear Type AH12 is designed and manufactured to fully comply with the requirements as specified in International
Standards and relevant customer specifications.
Standard
IEC 62271-1 High Voltage Switchgear.
I EC 62271-100 Alternating current circuit breakers.
IEC 62271-200 Alternating-current metal-enclosed switchgear for rated voltages higher than 1kV and less than or equal to 52 kV.
IEC 62271-102 Alternating current disconnectors and earthing switches.
IEC 60529 Degrees of protection provided by the enclosures (IP code).
Rated Voltage - 12 kV
Rated Insulation Level - 28/95 kVp
Rated Frequency - 50 Hz
Rated Short Time Withstand Current- 40 kA
Rated duration of Short -Circuit - 3 Sec
Rated Peak Withstand Current - 100 kA
Rated Current - IEC / Kuwait Ambient -
- Outgoing feeder -1000A/ 800A
-Incomer feeder -2000A/ 2000A.
-Bus Coupler - 3150A/3150A.
-Bus sectionalizer with transfer unit - 3150A/3150A.
Internal Arc Classification -AFLR-40kA-1sec (as applicable)
Materials kg %
Electronic - Cable 33,84 0,32
Electronic - Heating element 26,16 0,24
Electronic - Relay 40,31 0,38
Electronic - Switch 5,60 0,05
Electronic component 0,96 0,01
Plastic - Nylon (PA) 40,44 0,38
Plastic - Polyvinyl chloride (PVC) 61,72 0,58
Powder coating 169,40 1,58
Electronics 0,87 0,01
Metal 9591,12 89,38
Chemical 685,84 6,39
Others 2,35 0,02
Paper 10,55 0,10
Plastic - Polycarbonate (PC) 61,95 0,58
Total 10731,11 100,00
Packaging kg %
Packaging - Plastic 3,35 1,14
Packaging - Wood 291,76 98,86
Total incl. packaging 11026,22 100,00
Technical data:
DBB Switchgear type AH12 is manufactured at Al-Ahleia Switchgear manufacturing facility in the State of Kuwait.
12kV , 40 KA ,DBB Switchgear : 12kV , 40 KA ,DBB Switchgear : Bus 12kV , 40 KA ,DBB Switchgear : 12kV , 40 KA ,DBB Switchgear :
Product
Bus coupler Type - AH12 Sectionalizer + Transfer Type - AH12 Incomer Type - AH12 Outgoing Feeder Type - AH12
Market:
Average distribution to middle east and gulf cooperation council countries (300 km).
Reference service life, product
25 Years
3/13
Reference service life, building or construction works
N/A
LCA: Calculation rules
Declared unit:
1 pcs DBB Air insulated switchgear Type: AH12 - Comprising of Outgoing & Incoming feeders, Buscoupler & Bus sectionalizer with Transfer
Cut-off criteria:
All major raw materials and all the essential energy is included. The production processes for raw materials and energy flows with very small
amounts (less than 1%) are not included. These cut-off criteria do not apply for hazardous materials and substances.
Allocation:
The allocation is made in accordance with the provisions of EN 15804. Incoming energy and water and waste production in-house is allocated
equally among all products through mass allocation. Effects of primary production of recycled materials is allocated to the main product in which
the material was used. The recycling process and transportation of the material is allocated to this analysis.
Data quality:
Specific data for the product composition are provided by the manufacturer. The data represent the production of the declared product and were
collected for EPD development in the year of study. Background data is based on EPDs according to EN 15804 and different LCA databases. The
data quality of the raw materials in A1 is presented in the table below.
Materials Source Data quality Year
Supplier data +
Chemical ecoinvent 3.6 2019
database
Electronic - Cable Ecoinvent 3.6 Database 2019
Electronic - Heating element ecoinvent 3.6 Database 2019
Electronic - Relay ecoinvent 3.6 Database 2019
Supplier data +
Electronic - Relay ecoinvent 3.6 2019
database
Electronic - Switch ecoinvent 3.6 Database 2019
Electronic component ecoinvent 3.6 Database 2019
Electronics ecoinvent 3.6 Database 2019
Supplier data +
Electronics ecoinvent 3.6 2019
database
Metal ecoinvent 3.6 Database 2019
Metal Modified ecoinvent 3.6 Database 2019
Others ecoinvent 3.6 Database 2019
Packaging - Plastic ecoinvent 3.6 Database 2019
Packaging - Wood ecoinvent 3.6 Database 2019
Paper ecoinvent 3.6 Database 2019
Plastic - Nylon (PA) ecoinvent 3.6 Database 2019
Plastic - Polycarbonate (PC) ecoinvent 3.6 Database 2019
Plastic - Polyvinyl chloride (PVC) ecoinvent 3.6 Database 2019
Powder coating Ecoinvent 3.6 Database 2019
4/13
System boundaries (X=included, MND=module not declared, MNR=module not relevant)
Construction Beyond the system
Product stage Use stage End of life stage
installation stage boundaries
A1 A2 A3 A4 A5 B1 B2 B3 B4 B5 B6 B7 C1 C2 C3 C4 D
X X X X X X MND MND MND MND X MND X X X X X
System boundary:
Additional technical information:
A DBB switchgear unit comprises of two independent busbar systems separated by metallic barriers. The choice of power feed to/from which
busbar is achieved through disconnectors mounted in the Incomer feeders & Outgoing feeders. As the main advantage of a DBB system is the
reliability of the power system, Bus sectionalizer with Transfer & Buscoupler plays the role to ensure the power is transferred to the required bus.
Normally of the two busbar systems, one will be the working and other standby. When the working busbar needs maintenance or isolation,
depending on the location, bus CBs in sectionalizer & bus coupler can be used to switch all the load on the working bus to the standby so not to
interrupt the power supply.
Thus a DBB switchgear configuration always comes with the above varieties of outgoing feeder, incomer feeder, Buscoupler, Bus sectionalizer with
transfer in place.
waR slairetam tropsnarT gnirutcafunaM tropsnarT ylbmessA e​sU ecnanetniaM riapeR tnemecalpeR tnemhsibrufeR lanoitarepO ygrene esu lanoitarepO esu retaw -eD noitcurtsnoc noitilomed tropsnarT etsaW gnissecorp lasopsiD -yrevoceR-esueR laitnetop-gnilcyceR
5/13
LCA: Scenarios and additional technical information
The following information describe the scenarios in the different modules of the EPD.
Module A4 = Average distribution to middle east and gulf cooperation council countries (300 km).
Module A5 = Installation is performed by manual labor, with the use of electrical machines, that fall under the cut-off criteria of 1% and is
therefore neglected. Packaging of the final product consist of wooden pallet and plastic packaging.
Module B6 = The operational energy use of the switchgear is calculated based on the methodology provided in EPD Italy PCR -015 for
switchboards. To calculate the electricity use of the switchgear, the following scenario parameters have been applied for each component (outgoing
& Incoming feeder, Buscoupler & Bus sectionalizer with Transfer):
-Reference power consumption in Watts (Puse) = 1661.85 watt
-Standard year time (ty) = 8760 hours
-Use Time rate (a) = 99.5%
-Euse [kWh] = 362125
Module C1 = The de-installation of the switchgear is carried out manually, with the assistance of electrical tools. The energy consumption of
portable electrical devices (e.g., drills) is typically low, falling below the 1% cut-off criterion, and is therefore disregarded.
Module C2 = Transportation from building site to the waste treatment facility with an average distance of 300km.
Modules C3 and C4 = Waste treatment of the product follows the default values provided in EN 50693, Product Category Rules for life cycle
assessments of electronic and electrical products and systems, table G.4. This table specified how different types of raw materials used in A1 will
likely be treated during the end-of-life of the product. Waste treatments in C3 include material recycling and incineration with and without energy
recovery and fly ash extraction. Disposal in C4 consist of landfilling of different waste fractions and of ashes.
Module D = The recyclability of metals, plastics, and electronic components allows the producers a credit for the net scrap that is produced at the
end of a product’s life. The benefits from recycling of net scrap are described in formula from EN 15804:2012+A2:2019. Substitution of heat and
electricity generated by the incineration with energy recovery of plastic insulation and other parts is also calculated in module D.
Capacity utilisation Value
Transport from production place to user (A4) Distance (km) Fuel/Energy Consumption Unit
(incl. return) % (Liter/tonne)
Truck, 16-32 tonnes, EURO 6 (km) - Rest of World 38,8 % 300 0,044 l/tkm 13,20
Assembly (A5) Unit Value
Waste, wood, to average treatment - A5 including
kg 291,76
transport (kg)
Waste, packaging, plastic film (LDPE), to average
kg 3,35
treatment (kg)
Operational energy (B6) Unit Value
Electricity, medium voltage (kWh) - Middle East
kWh 362125
average
Capacity utilisation Value
Transport to waste processing (C2) Distance (km) Fuel/Energy Consumption Unit
(incl. return) % (Liter/tonne)
Truck, 16-32 tonnes, EURO 6 (km) - Rest of World 38,8 % 300 0,044 l/tkm 13,20
Waste processing (C3) Unit Value
Metal to recycling (kg) kg 7222,22
Waste treatment of plastic mixture, incineration
kg 455,88
with energy recovery and fly ash extraction (kg)
Waste treatment per kg used electronic
kg 100,44
components, manual seperation (kg)
Waste, Metals to recycling (kg) kg 15,98
Waste treatment per kg Non-hazardous waste,
kg 10,54
incineration with fly ash extraction - (kg)
Waste treatment per kg Emulsion Paint,
kg 169,40
hazardous waste incineration (kg)
Disposal (C4) Unit Value
Landfilling of Metal (kg) kg 2393,94
Landfilling of ashes from incineration of Plastic
kg 15,94
mixture, process per kg ashes and residues (kg)
Landfilling of plastic mixture (kg) kg 455,88
Landfilling of ashes from incineration of Non-
hazardous waste, process per kg ashes and kg 2,50
residues (kg)
Landfilling of ashes from incineration of Emulsion
Paint, hazardous waste incineration, process of kg 119,76
ashes and residues (kg)
Landfilling of hazardous waste (kg) kg 2,35
6/13
Benefits and loads beyond the system
Unit Value
boundaries (D)
Substitution of primary steel with net scrap (kg) kg 3241,60
Substitution of primary copper with net scrap (kg) kg 724,65
Substitution of primary Brass with net scrap (kg) kg 0,75
Substitution of primary aluminium with net scrap
kg 0,20
(kg)
Substitution of electricity (MJ) MJ 706,88
Substitution of thermal energy, district heating
MJ 10694,41
(MJ)
Substitution of primary other ferrous metals with
kg 15,98
net scrap (kg)
7/13
LCA: Results
The LCA results are presented below for the declared unit defined on page 2 of the EPD document.
Environmental impact
Indicator Unit A1-A3 A4 A5 B1 B6 C1 C2 C3 C4 D
GWP-total
kg CO2 -
7,07E+04 5,65E+02 4,50E+02 0 3,07E+05 0 5,65E+02 1,47E+03 1,23E+02 -5,40E+03
eq
GWP-fossil
kg CO2 -
7,01E+04 5,65E+02 8,12E+00 0 3,07E+05 0 5,65E+02 1,46E+03 1,23E+02 -5,38E+03
eq
GWP-biogenic
kg CO2 -
5,67E+02 2,20E-01 4,42E+02 0 2,68E+01 0 2,20E-01 7,31E+00 2,14E-02 -1,02E+01
eq
GWP-luluc
kg CO2 -
6,22E+01 2,07E-01 2,03E-03 0 1,03E+01 0 2,07E-01 1,24E-01 2,27E-02 -5,61E+00
eq
kg
ODP CFC11 - 6,58E-03 1,23E-04 1,27E-06 0 4,97E-02 0 1,23E-04 5,18E-05 1,28E-05 -4,52E+00
eq
mol H+
AP 2,32E+03 1,69E+00 6,35E-02 0 2,26E+03 0 1,69E+00 9,29E-01 4,21E-01 -3,09E+02
-eq
EP-FreshWater kg P -eq 2,10E+01 5,30E-03 9,46E-05 0 4,69E-01 0 5,30E-03 3,58E-03 1,20E-03 -2,19E+00
EP-Marine kg N -eq 1,27E+02 3,33E-01 2,74E-02 0 3,23E+02 0 3,33E-01 2,32E-01 2,00E-01 -1,58E+01
mol N -
EP-Terrestial 1,90E+03 3,72E+00 2,91E-01 0 3,54E+03 0 3,72E+00 2,50E+00 1,67E+00 -2,25E+02
eq
kg
POCP NMVOC 5,05E+02 1,39E+00 7,50E-02 0 1,02E+03 0 1,39E+00 7,22E-01 4,66E-01 -6,88E+01
-eq
ADP- kg Sb-
2,10E+01 1,52E-02 1,29E-04 0 3,10E-01 0 1,52E-02 1,81E-03 3,76E-04 -1,71E+00
minerals&metals1 eq
ADP-fossil1 MJ 8,52E+05 8,35E+03 9,34E+01 0 4,15E+06 0 8,35E+03 2,70E+03 1,09E+03 -4,66E+04
WDP1 m3 3,72E+05 2,72E+03 1,46E+02 0 1,51E+06 0 2,72E+03 1,14E+04 2,52E+04 2,69E+05
GWP-total = Global Warming Potential total; GWP-fossil = Global Warming Potential fossil fuels; GWP-biogenic = Global Warming Potential biogenic; GWP-luluc =
Global Warming Potential land use and land use change; ODP = Depletion potential of the stratospheric ozone layer; AP = Acidification potential, Accumulated
Exceedance; EP-freshwater = Eutrophication potential, fraction of nutrients reaching freshwater end compartment: EP-marine = Eutrophication potential, fraction of
nutrients reaching marine end compartment; EP-terrestrial = Eutrophication potential, Accumulated Exceedance; POCP = Formation potential of tropospheric ozone;
ADP-minerals&metals = Abiotic depletion potential for non-fossil resources; ADP-fossil = Abiotic depletion for fossil resources potential; WDP = Water (user)
deprivation potential, deprivation-weighted water consumption
"Reading example: 9,0 E-03 = 9,0*10-3 = 0,009"
*INA Indicator Not Assessed
1. The results of this environmental impact indicator shall be used with care as the uncertainties on these results are high or as there is limited experienced with the
indicator
Remarks to environmental impacts
8/13
Additional environmental impact indicators
Indicator Unit A1-A3 A4 A5 B1 B6 C1 C2 C3 C4 D
PM Disease incidence 7,18E-03 3,65E-05 7,78E-07 0 1,64E-02 0 3,65E-05 1,24E-05 7,74E-06 -9,11E-04
IRP2 kgBq U235 -eq 2,24E+03 3,47E+01 3,39E-01 0 1,24E+04 0 3,47E+01 1,24E+01 6,83E+00 -1,23E+01
ETP-fw1 CTUe 1,65E+07 6,77E+03 1,06E+02 0 1,53E+06 0 6,77E+03 9,64E+03 1,48E+06 -2,88E+06
HTP-c1 CTUh 5,26E-04 0,00E+00 1,17E-08 0 9,16E-05 0 0,00E+00 1,26E-07 1,23E-07 -5,51E-05
HTP-nc1 CTUh 3,26E-02 6,64E-06 5,62E-07 0 8,99E-04 0 6,64E-06 5,46E-06 2,55E-06 -2,87E-03
SQP1 dimensionless 3,86E+05 5,72E+03 5,36E+01 0 4,10E+05 0 5,72E+03 1,20E+03 2,25E+03 -4,22E+04
PM = Particulate Matter emissions; IRP = Ionizing radiation – human health; ETP-fw = Eco toxicity – freshwater; HTP-c = Human toxicity – cancer effects; HTP-nc =
Human toxicity – non cancer effects; SQP = Potential Soil Quality Index (dimensionless)
"Reading example: 9,0 E-03 = 9,0*10-3 = 0,009"
*INA Indicator Not Assessed
1. The results of this environmental impact indicator shall be used with care as the uncertainties on these results are high or as there is limited experienced with the
indicator
2. This impact category deals mainly with the eventual impact of low dose ionizing radiation on human health of the nuclear fuel cycle. It does not consider effects due
to possible nuclear accidents, occupational exposure nor due to radioactive waste disposal in underground facilities. Potential ionizing radiation from the soil, from
radon and from some construction materials is also not measured by this indicator.
9/13
Resource use
Indicator Unit A1-A3 A4 A5 B1 B6 C1 C2 C3 C4 D
PERE MJ 6,76E+04 9,45E+01 1,92E+00 0 1,30E+04 0 9,45E+01 5,26E+02 1,37E+02 -1,41E+04
PERM MJ 4,10E+03 0,00E+00 -4,05E+03 0 0,00E+00 0 0,00E+00 -4,57E+01 0,00E+00 0,00E+00
PERT MJ 7,17E+04 9,45E+01 -4,05E+03 0 1,30E+04 0 9,45E+01 4,80E+02 1,37E+02 -1,41E+04
PENRE MJ 8,46E+05 8,35E+03 9,34E+01 0 4,15E+06 0 8,35E+03 2,70E+03 1,09E+03 -4,66E+04
PENRM MJ 1,36E+04 0,00E+00 -1,42E+02 0 0,00E+00 0 0,00E+00 -1,34E+04 0,00E+00 0,00E+00
PENRT MJ 8,60E+05 8,35E+03 -4,89E+01 0 4,15E+06 0 8,35E+03 -1,07E+04 1,09E+03 -4,66E+04
SM kg 3,60E+03 0,00E+00 0,00E+00 0 0,00E+00 0 0,00E+00 0,00E+00 5,08E-02 5,06E+02
RSF MJ 5,46E+02 1,85E+00 5,60E-02 0 2,39E+02 0 1,85E+00 1,11E+01 2,88E+00 1,77E+02
NRSF MJ 1,27E+04 1,57E+01 6,32E-01 0 1,22E+03 0 1,57E+01 0,00E+00 3,71E+00 3,55E+03
FW m3 6,64E+02 9,34E-01 6,77E-02 0 7,09E+02 0 9,34E-01 2,35E+00 1,45E+00 -5,66E+01
PERE = Use of renewable primary energy excluding renewable primary energy resources used as raw materials; PERM = Use of renewable primary energy resources used
as raw materials; PERT = Total use of renewable primary energy resources; PENRE = Use of non renewable primary energy excluding non-renewable primary energy
resources used as raw materials; PENRM = Use of non renewable primary energy resources used as raw materials; PENRT = Total use of non renewable primary energy
resources; SM = Use of secondary materials; RSF = Use of renewable secondary fuels; NRSF = Use of non-renewable secondary fuels; FW = Net use of fresh water
"Reading example: 9,0 E-03 = 9,0*10-3 = 0,009"
*INA Indicator Not Assessed
10/13
End of life - Waste
Indicator Unit A1-A3 A4 A5 B1 B6 C1 C2 C3 C4 D
HWD kg 5,09E+02 7,54E-01 0,00E+00 0 3,71E+02 0 7,54E-01 0,00E+00 9,47E+01 -3,83E+01
NHWD kg 1,60E+04 4,01E+02 2,95E+02 0 4,36E+03 0 4,01E+02 1,05E+01 3,01E+03 -2,32E+03
RWD kg 2,72E+00 5,48E-02 0,00E+00 0 2,02E+01 0 5,48E-02 0,00E+00 6,24E-03 -1,24E-02
HWD = Hazardous waste disposed; NHWD = Non-hazardous waste disposed; RWD = Radioactive waste disposed
"Reading example: 9,0 E-03 = 9,0*10-3 = 0,009"
*INA Indicator Not Assessed
End of life - Output flow
Indicator Unit A1-A3 A4 A5 B1 B6 C1 C2 C3 C4 D
CRU kg 0,00E+00 0,00E+00 0,00E+00 0 0,00E+00 0 0,00E+00 0,00E+00 0,00E+00 0,00E+00
MFR kg 2,32E+03 0,00E+00 1,72E+00 0 0,00E+00 0 0,00E+00 7,24E+03 4,09E-02 -1,99E+01
MER kg 2,48E+02 0,00E+00 2,92E+02 0 0,00E+00 0 0,00E+00 6,36E+02 1,00E-03 -2,61E+00
EEE MJ 1,44E+02 0,00E+00 2,03E+02 0 0,00E+00 0 0,00E+00 7,01E+02 6,49E-02 -6,42E+00
EET MJ 2,17E+03 0,00E+00 3,07E+03 0 0,00E+00 0 0,00E+00 1,06E+04 9,82E-01 -9,72E+01
CRU = Components for re-use; MFR = Materials for recycling; MER = Materials for energy recovery; EEE = Exported energy electrical; EET = Exported energy thermal
"Reading example: 9,0 E-03 = 9,0*10-3 = 0,009"
*INA Indicator Not Assessed
Biogenic Carbon Content
Indicator Unit At the factory gate
Biogenic carbon content in product kg C 1,51E+00
Biogenic carbon content in accompanying packaging kg C 1,21E+02
Note: 1 kg biogenic carbon is equivalent to 44/12 kg CO2
11/13
Additional requirements
Greenhouse gas emissions from the use of electricity in the manufacturing phase
National production mix from import, low voltage (production of transmission lines, in addition to direct emissions and losses in grid) of applied
electricity for the manufacturing process (A3).
Electricity mix Source Amount Unit
Electricity, low voltage (kWh) - Kuwait ecoinvent 3.6 938,36 g CO2-eq/kWh
Dangerous substances
The product contains no substances given by the REACH Candidate list.
Indoor environment
Additional Environmental Information
Additional environmental impact indicators required in NPCR Part A for construction products
Indicator Unit A1-A3 A4 A5 B1 B6 C1 C2 C3 C4 D
GWPIOBC kg CO2 -eq 7,11E+04 5,65E+02 8,12E+00 0 3,07E+05 0 5,65E+02 1,45E+03 1,31E+02 -6,26E+03
GWP-IOBC: Global warming potential calculated according to the principle of instantaneous oxidation. In order to increase the transparency of biogenic carbon​
contribution to climate impact, the indicator GWP-IOBC is required as it declares climate impacts calculated according to the principle of instantaneous oxidation.​
GWP-IOBC is also referred to as GWP-GHG in context to Swedish public procurement legislation.
12/13
Bibliography
EN ISO 14025:2010. Environmental labels and declarations - Type III environmental declarations - Principles and procedures. International
Organization for Standardization.
ISO 14044:2006. Environmental management - Life cycle assessment - Requirements and guidelines. International Organization for
Standardization.
EN 15804:2012+A2:2019. Environmental product declaration - Core rules for the product category of construction products. European
Committee for Standardization.
ISO 21930:2017. Sustainability in buildings and civil engineering works - Core rules for environmental product declarations of construction
products. International Organization for Standardization.
EN 50693:2019. Product category rules for life cycle assessments of electronic and electrical products and systems. European Committee for
Standardization.
Ecoinvent v3, 2019. Allocation, cut-off by classification. Swiss Centre of Life Cycle Inventories.
Iversen et al., (2021). eEPD v2021.09, background information for EPD generator tool system verification, LCA.no. Report number: 07.21. System
verification report.
Ali & Graafland (2024). EPD generator for PCR EPD Italy 015 part B for switchboards, background information for EPD generator application and
LCA data, LCA.no. Report number: 14.24. PCR verification report.
EPD Italy (2020). PCR EPD Italy 007 Part A for electronic and electrical products and systems. EPD Italy. Version 3, issue 13-01-2023 and valid
until 19-01-2025.
EPD Italy (2020). PCR EPD Italy 015 Part B for switcboards. EPD Italy. Version 0, issue 23-02-2022 and valid until 24-09-2025.
Program operator and publisher Phone: +47 977 22 020
The Norwegian EPD Foundation e-mail: post@epd-norge.no
Post Box 5250 Majorstuen, 0303 Oslo, Norway web: www.epd-norge.no
Owner of the declaration: Phone: +965 24271000
Al-Ahleia Switchgear Co., k.s.c.c e-mail: ahleia@ahleiasg.com
, , Kuwait web: https://www.ahleiasg.com
Author of the Life Cycle Assessment Phone: +47 916 50 916
LCA.no AS e-mail: post@lca.no
Dokka 6A, 1671 Kråkerøy, Norway web: www.lca.no
Developer of EPD generator Phone: +47 916 50 916
LCA.no AS e-mail: post@lca.no
Dokka 6A, 1671 Kråkerøy, Norway web: www.lca.no
ECO Platform web: www.eco-platform.org
ECO Portal web: ECO Portal
13/13
