ENVIRONMENTAL-PRODUCT DECLARATION
as per ISO 14025 and EN 15804+A2
Owner of the Declaration dormakaba International Holding GmbH
Publisher Institut Bauen und Umwelt e.V. (IBU)
Programme holder Institut Bauen und Umwelt e.V. (IBU)
Declaration number EPD-DOR-20210151-CBA1-EN
Issue date 29/06/2021
Valid to 28/06/2026
Double cylinder - star cross, star, 20 and 8
dormakaba
www.ibu-epd.com | https://epd-online.com
General Information
dormakaba Double cylinder - star cross, star, 20 and 8
Programme holder Owner of the declaration
IBU – Institut Bauen und Umwelt e.V. dormakaba International Holding GmbH
Hegelplatz 1 DORMA Platz 1
10117 Berlin 58256 Ennepetal
Germany Germany
Declaration number Declared product / declared unit
EPD-DOR-20210151-CBA1-EN 1 piece of the product: star mechanical key system, consisting of the
following items:
- one star double cylinder
- one star reversible key
This declaration is based on the product category rules: Scope:
Building Hardware products, 01/08/2021 This EPD refers to a mechanical key system, including the star double
(PCR checked and approved by the SVR) cylinder and one star reversible key. This EPD is also representative for
the products: star cross, star, 20 and 8. The underlying life cycle
assessment is based on the entire life cycle of this specific master key
Issue date system manufacured by dormakaba. Data represents the year 2021.
29/06/2021
The various technical features are outlined in the Product chapter of this
EPD. The products are manufactured at the dormakaba production facility
in Wetzikon (Switzerland).
Valid to
The owner of the declaration shall be liable for the underlying information
28/06/2026 and evidence; the IBU shall not be liable with respect to manufacturer
information, life cycle assessment data and evidences.
The EPD was created according to the specifications of EN 15804+A2. In
the following, the standard will be simplified as EN 15804 bezeichnet.
Verification
The standard EN 15804 serves as the core PCR
Independent verification of the declaration and data according to ISO
14025:2011
internally X externally
Dipl.-Ing Hans Peters
(chairman of Institut Bauen und Umwelt e.V.)
Florian Pronold Dr.-Ing. Wolfram Trinius,
(Managing Director Institut Bauen und Umwelt e.V.) (Independent verifier)
1 Environmental-Product Declaration - dormakaba - Double cylinder - star cross, star, 20 and 8
Product
• Five to eight rows of pins with up to 26 simultaneously-
Product description/Product definition
usable pin positions.
Information about the enterprise
• Pins that make contact with the key are manufactured
Dormakaba stands for a broad offering of products, solutions
from wear-resistant hardened steel.
and services for smart and secure access to buildings and
• Key protected by patented characteristic.
rooms from a single source.
• Key of star cross with active protection against copies.
20 is a locking system, which is a patented system, registered
Product description/ Product definition
and factory produced.
star is the most advanced patented master key system. It offers
8 is a locking system, which is non patented and non registered
legal protection against commercial imitation. The registration
and with a possibility to assemble components at the dealer to
of individual locking system, and master key system with
be more flexible and faster to deliver to the end customer.
dormakaba ensures that keys cannot be ordered without
All systems are available with 22 mm Swiss round profile
authorization. Extensions or single parts can be ordered as
cylinders and 17 mm diameter Euro profile cylinders.
required.
All systems are classified according to the European locking
cylinder standards EN1303 and DIN18252. While the basic
This feature also applies for star cross and 20.
cylinder configuration already fulfills the attack resistance class
The system is ideal and can be used in both the private sector
B, the highest protection grade D is an option that can be
as for large and complex buildings with high security
achieved with integrated carbide steel inserts.
requirements. star cross, star and 20 can be equipped with
RFID transponder for integration in electronic access systems
from dormakaba.
star uses the dormakaba keylink planning method and has a
virtually unlimited number of locking combinations. For placing
the Please list the Technical Data according to the
mechanical key systems on the market in the European List in the chapter “Product group specific calculation rules”
Union/European Free Trade
Association (EU/EFTA, with the exception of Switzerland) the
following legal provisions
apply: Example:
Technical
• DIN EN 1303: 2015-08
Data for Locking Cylinders acc. to the classification in EN
Building
1303: Delivery
Hardware - Cylinders for locks - Requirements and test
status:
methods
• DIN 18252: 2018-05Profile cylinders for door locks –
Terminology, dimensions,
requirements, test methods and marking
The declared mechanical key system includes one Swiss round
profile double cylinder and one key, packaging and service
• Restriction of instruction with a weight of 0,259 kg.
Hazardous Substances (RoHS)
Base materials/Ancillary materials
Directive on
the restriction of the use of certainhazardous For the main
substances in electrical and electronic equipment product components, the star
(RoHS), Directive (EU) No 2011/65. In double cylinder and star
addition, the mechanical cylinders meet the material reversible key the composition of the product is the following.
requirements of the RoHS Same product
2011/65/EU directive composition applies for star cross, star, 20 and 8:
Application
Reversible
mechanical double cylinder can be used in both residential as
well as in the
commercial segment and in small and simple as well as inlarge
and
complex applications, thanks to its versatility. Nearly limitless
application
options are possible.
Technical Data
star cross and star are locking systems, which fulfill even the
The reversible
most challenging requirements. Both systems offer exceptional
mechanical double cylinder and reversible key contain partial
security thanks to:
articles which contain substances listed
in the Candidate List of REACH Regulation 1907/2006/EC
2 Environmental-Product Declaration - dormakaba - Double cylinder - star cross, star, 20 and 8
(date: 19.01.2021) https://echa.europa.eu/de/home.
exceeding 0.1 percentage by mass: yes
Environment and health during use
Reference service life
The
life cycle (security and function) of a lock cylinder is about 15
• Lead (Pb): 7439-92-1 (CAS-No.) years,
is included in some of the alloys used. The depending on the application frequency of use. The cylinders
concentration of lead in each are tested to 100,000 (EN1303) locking cycles minimum. This
individual alloy does not exceed 4.0% (by mass). corresponds to approximately 18 locking cycles per day for 15
years. In case of extensions parts are available for a long
The candidate lifetime. Availability
list can be found on the /ECHA/ website address: for over 30 years is secured.
LCA: Calculation rules
— A4, transport to the building site;
Declared Unit — A5, installation into the building;
The declared unit is 1 piece of the product: kaba star. including provision of all materials, products and
Declared unit energy, as well as waste processing up to the end-ofwaste
state or disposal of final residues during the
Name Value Unit
construction process stage.
Declared unit 1 piece/product
Conversion factor to 1 kg (mass of
0.259 -
declared unit) End-of-life stage– Modules C1-C4 and D
The end-of-life stage includes:
For IBU core EPDs (where clause 3.6 is part of the EPD): for
— C1, de-construction, demolition:
average EPDs, an estimate of the robustness of the LCA
— C2, transport to waste processing;
values must be made, e.g. concerning variability of the
— C3, waste processing for reuse, recovery and/or
production process, geographical representativeness and the
recycling;
influence of background data and preliminary products
— C4, disposal;
compared to the environmental impacts caused by actual
including provision and all transport, provision of all
production.
materials, products and related energy and water use.
Module D (Benefits and loads beyond the system
System boundary boundary) includes:
The type of EPD is: cradle to gate with options, — D, recycling potentials, expressed as net impacts
modules C1–C4, and module D and benefits.
(A1–A3 + C + D and additional modules: A4 + A5)
Geographic Representativeness
Production - Module A1-A3
The product stage includes: Land or region, in which the declared product system is
— A1, raw material extraction, processing and manufactured, used or handled at the end of the product´s
mechanical treatments, processing of secondary lifespan: Switzerland
material input (e.g. recycling processes),
— A2, transport to the manufacturer,
Comparability
— A3, manufacturing and assembly
Basically, a comparison or an evaluation of EPD data is only
including provision of all materials, products and
possible if all the data sets to be compared were created
energy, as well as waste processing up to the end-of
according to EN 15804 and the building context, respectively
waste state.
the product-specific characteristics of performance, are taken
into account. Background database: GaBi ts
software, SP40.
Construction stage - Modules A4-A5
The construction process stage includes:
LCA: Scenarios and additional technical information
Characteristic product properties Note: 1 kg of biogenic carbon is equivalent to 44/12 kg of CO2.
Information on biogenic carbon
Information on describing the biogenic Carbon Content at
The biogenic carbon content quantifies the amount of biogenic
factory gate
carbon in a construction product leaving the factory gate, and it
Name ValueUnit
shall be separately declared for the product and for any
accompanying packaging. Biogenic carbon content in accompanying kg
0.02
If the total mass of biogenic carbon containing materials is less packaging C
than 5 % of the total mass of the product and accompanying
packaging, the declaration of biogenic carbon content may be The following technical scenario information is required for the
omitted. The mass of packaging containing biogenic carbon declared modules.
shall always be declared.
Transport to the building site (A4)
3 Environmental-Product Declaration - dormakaba - Double cylinder - star cross, star, 20 and 8
Name Value Unit The same holds for a service life declared by the manufacturer.
Corresponding information related to in-use conditions needs
Litres of fuel (per piece) 0.0015l/100km
not be provided if a service life taken from the list on service life
Transport distance 100 km
by BNB is declared.
Capacity utilisation (including empty runs)
55 %
average
End of life (C1-C4)
Installation into the building (A5) C1: The product dismantling from the building is done manually
without environmental burden.
Name ValueUnit
Output substances following waste treatment on Name Value Unit
0.045 kg
site (packaging waste) Collected separately waste type 0.214 kg
The product is disassembled in a recycling process.
In case a reference service life according to applicable ISO Material recycling is then assumed for the metals. The plastic
standards is declared then the assumptions and in-use components are assumed to be incinerated with energy
conditions underlying the determined RSL shall be declared. In recovery.
addition, it shall be stated that the RSL applies for the reference
conditions only. Reuse, recovery and/or recycling potentials (D),
relevant scenario information
Collection rate is 100%.
4 Environmental-Product Declaration - dormakaba - Double cylinder - star cross, star, 20 and 8
LCA: Results
Disclaimer EP-freshwater: This indicator has been calculated as “kg P eq” as required in the characterization
model (EUTREND model, Struijs et al., 2009b, as implemented in ReCiPe;
http://eplca.jrc.ec.europa.eu/LCDN/developerEF.xhtml).
DESCRIPTION OF THE SYSTEM BOUNDARY (X = INCLUDED IN LCA; ND = MODULE OR INDICATOR NOT DECLARED; MNR =
MODULE NOT RELEVANT)
BENEFITS
AND LOADS
CONSTRUCTION
BEYOND
PRODUCT STAGE PROCESS USE STAGE END OF LIFE STAGE
THE SYSTEM
STAGE
BOUNDARIE
S
la ire ta m w a Ry lp p u s tro p s n a rT g n iru tc a fu n a M e h t m o rf tro p s n a rTe tis e h t o t e ta g y lb m e s s A e s U e c n a n e tn ia M ria p e R tn e m e c a lp e R tn e m h s ib ru fe R y g re n e la n o ita re p Oe s u re ta w la n o ita re p Oe s u n o itc u rts n o c -e Dn o itilo m e d tro p s n a rT g n is s e c o rp e ts a W la s o p s iD -e s u e R-y re v o c e R-g n ilc y c e Rla itn e to p
A1 A2 A3 A4 A5 B1 B2 B3 B4 B5 B6 B7 C1 C2 C3 C4 D
X X X X X MND MND MNR MNR MNR MND MND X X X MND X
RESULTS OF THE LCA - ENVIRONMENTAL IMPACT according to EN 15804+A2: 1 piece, Double cylinder - star cross, star, 20
and 8
Parameter Unit A1-A3 A4 A5 C1 C2 C3 D
GWP-total kg CO 2 eq 3.82E-01 2.26E-03 7.05E-02 0 9.36E-04 3.56E-03 -1.03E-01
GWP-fossil kg CO 2 eq 3.92E-01 2.16E-03 1.66E-02 0 8.94E-04 3.56E-03 -1.03E-01
GWP-biogenic kg CO 2 eq -1.02E-02 1E-04 5.39E-02 0 4.13E-05 8.29E-08 2.24E-04
GWP-luluc kg CO 2 eq 6.64E-04 5.15E-08 1.77E-06 0 2.13E-08 2.01E-07 -1.56E-04
ODP kg CFC11 eq 1.58E-12 2.29E-19 1.77E-17 0 9.44E-20 1.79E-18 -4.48E-16
AP mol H+ eq 3.47E-03 2.17E-06 1.82E-05 0 8.95E-07 6.33E-07 -9.21E-04
EP-freshwater kg P eq 1.61E-06 4.63E-10 3.18E-09 0 1.91E-10 2.86E-10 -5.9E-08
EP-marine kg N eq 3.09E-04 6.89E-07 6.2E-06 0 2.85E-07 1.43E-07 -6.35E-05
EP-terrestrial mol N eq 3.3E-03 7.66E-06 8.21E-05 0 3.17E-06 2.89E-06 -6.72E-04
kg NMVOC
POCP 1.01E-03 1.95E-06 1.65E-05 0 8.05E-07 3.95E-07 -2.29E-04
eq
ADPE kg Sb eq 1.29E-04 6.49E-11 2.63E-10 0 2.68E-11 2.46E-11 -2.07E-05
ADPF MJ 5.07E+00 3.07E-02 2.45E-02 0 1.27E-02 1.65E-03 -1.19E+00
m3 world eq
WDP 2.23E-01 4.24E-06 8.42E-03 0 1.75E-06 3.64E-04 -4.07E-02
deprived
GWP = Global warming potential; ODP = Depletion potential of the stratospheric ozone layer; AP = Acidification potential of land and water; EP =
Eutrophication potential; POCP = Formation potential of tropospheric ozone photochemical oxidants; ADPE = Abiotic depletion potential for non-fossil
resources; ADPF = Abiotic depletion potential for fossil resources; WDP = Water (user) deprivation potential)
RESULTS OF THE LCA - INDICATORS TO DESCRIBE RESOURCE USE according to EN 15804+A2: 1 piece, Double cylinder -
star cross, star, 20 and 8
Parameter Unit A1-A3 A4 A5 C1 C2 C3 D
PERE MJ 1.3E+01 9.68E-05 4.73E-01 0 4E-05 4.29E-04 -1.63E-01
PERM MJ 4.68E-01 0 -4.68E-01 0 0 0 0
PERT MJ 1.35E+01 9.68E-05 5.01E-03 0 4E-05 4.29E-04 -1.63E-01
PENRE MJ 4.77E+00 3.07E-02 2.83E-01 0 1.27E-02 4.82E-02 -1.19E+00
PENRM MJ 3.05E-01 0 -2.58E-01 0 0 -4.66E-02 0
PENRT MJ 5.08E+00 3.07E-02 2.45E-02 0 1.27E-02 1.65E-03 -1.19E+00
SM kg 1.93E-01 0 0 0 0 0 0
RSF MJ 0 0 0 0 0 0 0
NRSF MJ 0 0 0 0 0 0 0
FW m3 5.24E-03 1.74E-07 1.99E-04 0 7.17E-08 8.71E-06 -9.36E-04
PERE = Use of renewable primary energy excluding renewable primary energy resources used as raw materials; PERM = Use of renewable primary
energy resources used as raw materials; PERT = Total use of renewable primary energy resources; PENRE = Use of non-renewable primary energy
excluding non-renewable primary energy resources used as raw materials; PENRM = Use of non-renewable primary energy resources used as raw
materials; PENRT = Total use of non-renewable primary energy resources; SM = Use of secondary material; RSF = Use of renewable secondary fuels;
NRSF = Use of non-renewable secondary fuels; FW = Use of net fresh water
RESULTS OF THE LCA – WASTE CATEGORIES AND OUTPUT FLOWS according to EN 15804+A2:
1 piece, Double cylinder - star cross, star, 20 and 8
Parameter Unit A1-A3 A4 A5 C1 C2 C3 D
HWD kg 3.89E-08 2.98E-12 5.27E-11 0 1.23E-12 6.29E-12 -2.56E-08
NHWD kg 8.28E-02 3.14E-06 3.32E-03 0 1.3E-06 3.7E-04 -2.02E-02
RWD kg 2.51E-04 3.3E-08 1.18E-06 0 1.36E-08 6.12E-08 -2.62E-05
5 Environmental-Product Declaration - dormakaba - Double cylinder - star cross, star, 20 and 8
CRU kg 0 0 0 0 0 0 0
MFR kg 0 0 0 0 0 2.13E-01 0
MER kg 0 0 0 0 0 0 0
EEE MJ 7.94E-02 0 1.12E-01 0 0 0 0
EET MJ 1.44E-01 0 2.17E-01 0 0 0 0
HWD = Hazardous waste disposed; NHWD = Non-hazardous waste disposed; RWD = Radioactive waste disposed; CRU = Components for re-use;
MFR = Materials for recycling; MER = Materials for energy recovery; EEE = Exported electrical energy; EET = Exported thermal energy
RESULTS OF THE LCA – additional impact categories according to EN 15804+A2-optional:
1 piece, Double cylinder - star cross, star, 20 and 8
Parameter Unit A1-A3 A4 A5 C1 C2 C3 D
Disease
PM 2.96E-08 1.14E-11 1.2E-10 0 4.7E-12 8.08E-12 -8.67E-09
incidence
IR kBq U235 eq 3.73E-02 4.71E-06 1.66E-04 0 1.95E-06 5.52E-06 -5.38E-03
ETP-fw CTUe 3.71E+00 2.18E-02 1.09E-02 0 8.99E-03 6.19E-04 -5.23E-01
HTP-c CTUh 5.01E-09 4.09E-13 6.68E-13 0 1.69E-13 5.36E-14 -5.93E-11
HTP-nc CTUh 1.38E-08 1.75E-11 4.22E-11 0 7.23E-12 5.43E-12 -2.94E-09
SQP SQP 9.5E+00 7.89E-05 6.75E-03 0 3.26E-05 4.94E-04 -5.64E-01
PM = Potential incidence of disease due to PM emissions; IR = Potential Human exposure efficiency relative to U235; ETP-fw = Potential comparative
Toxic Unit for ecosystems; HTP-c = Potential comparative Toxic Unit for humans (cancerogenic); HTP-nc = Potential comparative Toxic Unit for humans
(not cancerogenic); SQP = Potential soil quality index
Disclaimer 1 – for the indicator “Potential Human exposure efficiency relative to U235”. This impact category deals mainly with the
eventual impact of low dose ionizing radiation on human health of the nuclear fuel cycle. It does not consider effects due to possible
nuclear accidents, occupational exposure nor due to radioactive waste disposal in underground facilities. Potential ionizing radiation
from the soil, from radon and from some construction materials is also not measured by this indicator.
Disclaimer 2 – for the indicators “abiotic depletion potential for non-fossil resources”, “abiotic depletion potential for fossil resources”,
“water (user) deprivation potential, deprivation-weighted water consumption”, “potential comparative toxic unit for ecosystems”,
“potential comparative toxic unit for humans – cancerogenic”, “Potential comparative toxic unit for humans - not cancerogenic”,
“potential soil quality index”. The results of this environmental impact indicator shall be used with care as the uncertainties on these
results are high or as there is limited experienced with the indicator.
References
DIN EN 1303: 2015-08 und Umwelt e.V. Version 1., Berlin: Institut Bauen und Umwelt
Building Hardware - Cylinders for locks - Requirements and test e.V., 2016. www.ibu-epd.com
methods
GaBi ts software
DIN 18252: 2018-05 Sphera Solutions GmbH Gabi Software System and Database
Profile cylinders for door locks – Terminology, dimensions, for Life Cycle Engineering 1992-2020 Version 10.0.0.71
requirements, test methods and marking University of Stuttgart Leinfelden-Echterdingen
EN 15804:2019+A2 GaBi ts documentation
EN 15804:2019+A2 (in press), Sustainability of construction
works — Environmental Product Declarations — Core rules for GaBi life cycle inventory data documentation (https://www.gabi-
the product category of construction products. software.com/support/gabi/gabidatabase- 2020-lci-
documentation/).
ISO 14025:2011-10
DIN EN ISO 14025:2011-10, Environmental labels and LCA-tool dormakaba
declarations — Type III environmental declarations — LCA tool, version 1.0.
Principles and procedures. Developed by Sphera Solutions GmbH
Registration, Evaluation, Authorisation and Restriction of PCR Part A
Chemicals (REACH) PCR – Part A: Calculation Rules for the Life Cycle Assessment
Regulation (EC) No 1907/2006 of the European Parliament and and Requirements on the Project Re-port according to EN
of the Council on the Registration, Evaluation, Authorisation 15804+A2:2019, Version 1.0, Institut Bauen und Umwelt e.V.,
and Restriction of Chemicals (REACH). www.ibu-epd.com.
Restriction of Hazardous Substances (RoHS) PCR Part B
Directive on the restriction of the use of certain hazardous PCR – Part B: Requirements on the EPD for Electronic and
substances in electrical and electronic equipment (RoHS), physical Access Control Systems , version 1.2, Institut Bauen
Directive (EU) No 2011/65. und Umwelt e.V., www.ibu-epd.com, 2017.
The literature referred to in the Environmental Product
Further References Declaration must be listed in full.Standards already fully quoted
in the EPD do not need to be listed here again.
IBU The current version of PCR Part A and PCR Part B of the PCR
Institut Bauen und Umwelt e.V.: General Programme document on which they are based must be referenced.
Instructions for the Preparation of EPDs at the Institut Bauen
6 Environmental-Product Declaration - dormakaba - Double cylinder - star cross, star, 20 and 8
Publisher
Institut Bauen und Umwelt e.V. +49 (0)30 3087748- 0
Hegelplatz 1 info@ibu-epd.com
10117 Berlin www.ibu-epd.com
Germany
Programme holder
Institut Bauen und Umwelt e.V. +49 (0)30 3087748- 0
Hegelplatz 1 info@ibu-epd.com
10117 Berlin www.ibu-epd.com
Germany
Author of the Life Cycle Assessment
Sphera Solutions GmbH +49 711 341817-0
Hauptstraße 111- 113 info@sphera.com
70771 Leinfelden-Echterdingen www.sphera.com
Germany
Owner of the Declaration
dormakaba International Holding GmbH +49 2333 793-0
DORMA Platz 1 info.de@dormakaba.com
58256 Ennepetal www.dormakaba.com
Germany
7 Environmental-Product Declaration - dormakaba - Double cylinder - star cross, star, 20 and 8
