ENVIRONMENTAL PRODUCT DECLARATION
as per ISO 14025 and EN 15804+A2
Owner of the Declaration
Programme holder Institut Bauen und Umwelt e.V. (IBU)
Publisher Institut Bauen und Umwelt e.V. (IBU)
Declaration number EPD-DUP-20220296-CBA1-EN
Issue date 13.12.2022
Valid to 12.12.2027
DuPont™ AirGuard® Air & Vapour Control Layer 5816X
DuPont de Nemours (Luxembourg) s.à.r.l.
www.ibu-epd.com | https://epd-online.com
Umwelt Produktdeklaration Name des Herstellers – Name des Produkts
General Information
DuPont de Nemours (Luxembourg) s.à.r.l. DuPont™ AirGuard® Air & Vapour
Control Layer 5816X
Programme holder Owner of the declaration
IBU – Institut Bauen und Umwelt e.V. DuPont de Nemours (Luxembourg) s.à.r.l.
Hegelplatz 1 Rue Général Patton
10117 Berlin L-2984 Contern
Germany Luxembourg
Declaration number Declared product / declared unit
EPD-DUP-20220296-CBA1-EN 1 m² DuPont™ AirGuard® Air & Vapour Control Layer
5816X
This declaration is based on the product Scope:
category rules: This document applies to DuPont™ AirGuard® Air &
False ceiling and underlay sheeting, 11.2017 Vapour Control Layer 5816X, made of glass fibre,
(PCR checked and approved by the SVR) aluminium and adhesive. The declared unit weight is
171.5 g/m2. LCA data were compiled using production
data for the year 2021, as well as for the year 2019 for
Issue date
the finishing processing (used for EPDs of Tyvek®
13.12.2022
products published in 2021). The declaration holder is
responsible for the underlying data and its verification.
Valid to
12.12.2027
The owner of the declaration shall be liable for the
underlying information and evidence; the IBU shall not
be liable with respect to manufacturer information, life
cycle assessment data and evidences.
The EPD was created according to the specifications
of EN 15804+A2. In the following, the standard will be
simplified as EN 15804.
Verification
The standard EN 15804 serves as the core PCR
Independent verification of the declaration and data
according to ISO 14025:2011
Dipl. Ing. Hans Peters internally x externally
(chairman of Institut Bauen und Umwelt e.V.)
Dr. Alexander Röder Vito D'Incognito
(Managing Director Institut Bauen und Umwelt e.V.)) (Independent verifier)
Product
Product description/Product definition Application
DuPont™ AirGuard® A2 FR AVCL is a fire-retardant This product is used on the warm side of the building
airtight vapour control layer for use within the internal envelope. It will provide a barrier to water vapour and
lining of roof, ceiling and wall systems. Enhancing the air movement. Additional features:
building fabric in terms of airtightness, energy • Fire-retardant. Reaction to fire: A2-s1, d0 to EN
efficiency and moisture management, improving indoor 13501-1: 2007+A1:2009
air quality and providing exceptional fire safety to the • AirGuard® A2 FR AVCL and DuPont™ AirGuard®
building and its occupants. FR System tape is tested and classified for free-span,
For the placing on the market of the product in the on mineral wool slab, gypsum plasterboard or fibre
European Union/European Free Trade Association cement board
(EU/EFTA) (with the exception of Switzerland) • Suitable for all building types, heights and proximities
Regulation (EU) No. 305/2011 (CPR) applies. The • High vapour resistance, limiting interstitial
product needs a declaration of performance taking into condensation
consideration EN 13984: 2013, Plastic and rubber • Suitable for high humidity buildings, such as
vapour control layers and the CE-marking. swimming pool halls etc
For the application and use the respective national • Thermal benefit in combination with a cavity due to
provisions apply. the low emissivity/reflective surface
Technical Data
2 Environmental Product Declaration DuPont de Nemours (s.à.r.l.) – DuPont™ AirGuard® Air & Vapour Control Layers
(5816X)
essential characteristics according to EN 13984: 2013,
Constructional data Plastic and rubber vapour control layers
The properties given below correspond to nominal
values, as declared in the Technical Data Sheet of the For more information please refer to: https://energy-
product. There is nevertheless an intrinsic variability for efficiency.dupont.com/products/
these properties, which explains the small difference
between the grammage declared below and the weight Base materials/Ancillary materials
used for the LCA calculation. The product is made of glass fibre (49 % of product
weight), aluminium (47 % of product weight) and
Name Value Unit adhesive (4 % of product weight).
Product designation acc. to EN
A type
13984 This product/article/at least one partial article contains
Grammage acc. to EN 1849-2 0.1715 kg/m2 substances listed in the candidate list
Resistance to water penetration (08.07.2022) exceeding 0.1 percentage by mass: no.
Pass -
acc. to EN 1928 (class)
Water vapor diffusion equivalent Reference service life
air layer thickness acc. to EN 4900 m The service life is assumed to be 30 years, even if
1931 longer lifetime can be obtained for membranes out of
Maximum tensile force acc. to EN plastic or elastomers (40 years according to BNB
800 N/50mm
12311-1 http://www.nachhaltigesbauen.de/baustoff-und-
Elongation acc. to EN 12311-1 4 % gebaeudedaten/nutzungsdauern-von-bauteilen.html).
Tear Resistance (nail) acc. to EN Since the whole lifecycle of the product is not
12310-1 (MD-XD) 170 - 150 N/mm considered and for sake of compliance to EN
15804+A2 (2019), the functional unit does not have to
Water vapour permeability after
be declared. Instead, the declaration unit is 1 m2 of the
ageing acc. to EN 13984, EN Pass
envelope.
1931
Performance data of the product in accordance with
the declaration of performance with respect to its
LCA: Calculation rules
Declared Unit were not older than 10 years. A proxy was used for the
This declaration applies to 1 m2 of DuPont™ adhesive.
AirGuard® Air & Vapour Control Layer 5816X, with a
declared unit weight of 171.5 g/m2. The representativeness can be classified as very good
for all the foreground data, and for most of the
Declared unit and mass reference background data.
Name Value Unit
Declared unit 1 m2 The GaBi database (Sphera Solutions GmbH, 2022.1)
Grammage 0.1715 kg/m2 was used to model background data.
Layer thickness 0.00015 m
Primary production data were collected to model the System boundary
two production steps for manufacturing (A1-A3). Type of EPD: Cradle-to-gate (with options)
Manufacturing data are representative for the years The system boundaries of the EPD follow the modular
2019 (finishing process) and 2021; the product is construction system as described by EN 15804.
manufactured in Finland and Germany. All energy and The LCA considers the following modules:
materials flows were considered. Only a few material · A1-A3: Manufacturing of pre-products,
flows were excluded from the modelling, but the sum of packaging, ancillary materials, transport to the factory
their weight did not exceed 1 % of the total input mass. and production, with the associated energy supply and
Manufacturing of the production machines and waste handling
systems and associated infrastructure were not taken · A4: Transport to the construction site
into account for the life cycle assessment. · A5: Installation into the building including
disposal of packaging
Transport to the construction site (A4) is based on · C4: Waste disposal, namely incineration
market shares of 2021 at country level, provided by · D: Potential for reuse, recovery and/or recycling
DuPont Luxembourg s.à.r.l., to cover at least 90 % of including benefits for product incineration from module
the sales. Eurostat data representative of 2019 were C4
used to model the shares between the packaging
disposal routes during the installation into the building Comparability
(A5). Regarding possible off-cuts during installation, Basically, a comparison or an evaluation of EPD data
the amount is lower than 5 % and therefore neglected. is only possible if all the data sets to be compared
were created according to EN 15804 and the building
Regarding background data, the Finish and German context, respectively the product-specific
electricity grid mix were applied to the production characteristics of performance, are taken into account.
plants in these countries. Other background data were
specific to Germany or the European average and
3 Environmental Product Declaration DuPont de Nemours (s.à.r.l.) – DuPont™ AirGuard® Air & Vapour Control Layers
(5816X)
LCA: Scenarios and additional technical information
Characteristic product properties
Information on biogenic carbon
The product does not contain biogenic carbon.
Information on describing the biogenic Carbon
Content at factury gate
Name Value Unit
Biogenic Carbon Content in
0.0037 kg C
accompanying packaging
Transport to the building site (A4)
Name Value Unit
Transport distance (truck) 1099 km
Transport distance (container
333 km
ship)
Installation into the building (A5)
Name Value Unit
Cardboard/paper waste to landfill 2.66E-04 kg
Cardboard/paper waste to incineration 2.84E-04 kg
Wood waste to landfill 2.74E-04 kg
Wood waste to incineration 2.26E-04 kg
Plastic waste to landfill 2.47E-05 kg
Plastic waste to incineration 3.94E-05 kg
End of life (C1-C4)
Name Value Unit
Collected as mixed construction
0.1715 kg
waste
Energy recovery 0.1715 kg
4 Environmental Product Declaration DuPont de Nemours (s.à.r.l.) – DuPont™ AirGuard® Air & Vapour Control Layers
(5816X)
LCA: Results
The results displayed below apply to 1 m² of DuPont™ AirGuard® Air & Vapour Control Layer 5816X, with a
declared unit weight of 171.5 g/m².
DESCRIPTION OF THE SYSTEM BOUNDARY (X = INCLUDED IN LCA; ND = MODULE OR INDICATOR NOT
DECLARED; MNR = MODULE NOT RELEVANT)
BENEFITS AND
CONSTRUCTI LOADS
PRODUCT STAGE ON PROCESS USE STAGE END OF LIFE STAGE BEYOND THE
STAGE SYSTEM
BOUNDARIES
5 Environmental Product Declaration DuPont de Nemours (s.à.r.l.) – DuPont™ AirGuard® Air & Vapour Control Layers
(5816X)
lairetam
waR
ylppus tropsnarT
gnirutcafunaM
eht
morf
tropsnarT
etis
eht
ot
etag
ylbmessA esU
ecnanetniaM
riapeR
tnemecalpeR tnemhsibrufeR
ygrene
lanoitarepO esu
retaw
lanoitarepO esu
noitcurtsnoc-eD
noitilomed tropsnarT
gnissecorp
etsaW
lasopsiD -esueR -yrevoceR -gnilcyceR laitnetop
A1 A2 A3 A4 A5 B1 B2 B3 B4 B5 B6 B7 C1 C2 C3 C4 D
X X X X X ND ND MNR MNR MNR ND ND ND ND ND X X
RESULTS OF THE LCA - ENVIRONMENTAL IMPACT according to EN 15804+A2: 1 m2 DuPont™
AirGuard® 5816X
Core Indicator Unit A1-A3 A4 A5 C4 D
Global warming potential - total [kg CO2-Eq.] 1.18E+0 1.68E-2 1.93E-3 5.53E-1 -3.24E-1
Global warming potential - fossil fuels [kg CO2-Eq.] 1.16E+0 1.65E-2 1.56E-4 5.53E-1 -3.22E-1
Global warming potential - biogenic [kg CO2-Eq.] 1.41E-2 2.68E-4 1.77E-3 -3.28E-5 -1.22E-3
GWP from land use and land use change [kg CO2-Eq.] 5.32E-4 9.09E-5 2.32E-8 0.00E+0 -2.43E-5
Depletion potential of the stratospheric ozone layer [kg CFC11-Eq.] 6.72E-12 1.01E-15 1.47E-16 3.64E-10 -1.31E-12
Acidification potential, accumulated exceedance [mol H+-Eq.] 5.98E-3 1.15E-4 4.00E-7 7.29E-5 -3.26E-4
Eutrophication, fraction of nutrients reaching freshwater
[kg P-Eq.] 1.21E-6 4.88E-8 3.35E-9 1.32E-9 -2.74E-7
end compartment
Eutrophication, fraction of nutrients reaching marine end
[kg N-Eq.] 9.54E-4 5.24E-5 1.70E-7 1.25E-5 -1.00E-4
compartment
Eutrophication, accumulated exceedance [mol N-Eq.] 1.04E-2 5.80E-4 1.65E-6 2.91E-4 -1.08E-3
Formation potential of tropospheric ozone photochemical
[kg NMVOC-Eq.] 2.93E-3 1.03E-4 6.67E-7 3.65E-5 -2.85E-4
oxidants
Abiotic depletion potential for non-fossil resources [kg Sb-Eq.] 1.35E-7 1.38E-9 5.05E-12 7.78E-15 -3.53E-8
Abiotic depletion potential for fossil resources [MJ] 1.58E+1 2.24E-1 8.11E-4 1.06E-1 -5.36E+0
Water (user) deprivation potential, deprivation-weighted [m³ world-Eq
2.35E-1 1.47E-4 1.05E-4 4.86E-2 -2.06E-2
water consumption (WDP) deprived]
RESULTS OF THE LCA - INDICATORS TO DESCRIBE RESOURCE USE according to EN 15804+A2: 1 m2
DuPont™ AirGuard® 5816X
Indicator Unit A1-A3 A4 A5 C4 D
Renewable primary energy as energy carrier [MJ] 6.12E+0 1.24E-2 1.03E-4 2.70E-3 -9.08E-1
Renewable primary energy resources as material utilization [MJ] 3.36E-4 6.83E-14 6.33E-15 3.20E-6 -6.90E-11
Total use of renewable primary energy resources [MJ] 6.12E+0 1.24E-2 1.03E-4 2.70E-3 -9.08E-1
Non-renewable primary energy as energy carrier [MJ] 1.58E+1 2.24E-1 8.12E-4 1.06E-1 -5.36E+0
Non-renewable primary energy as material utilization [MJ] 3.32E-4 7.67E-6 1.74E-8 3.07E-10 -1.25E-4
Total use of non-renewable primary energy resources [MJ] 1.58E+1 2.24E-1 8.12E-4 1.06E-1 -5.36E+0
Use of secondary material [kg] 4.86E-3 0.00E+0 0.00E+0 0.00E+0 0.00E+0
Use of renewable secondary fuels [MJ] 5.65E-8 0.00E+0 0.00E+0 0.00E+0 0.00E+0
Use of non-renewable secondary fuels [MJ] 6.23E-7 0.00E+0 0.00E+0 0.00E+0 0.00E+0
Use of net fresh water [m³] 1.49E-2 1.40E-5 1.50E-6 0.00E+0 -8.77E-4
RESULTS OF THE LCA – WASTE CATEGORIES AND OUTPUT FLOWS according to EN 15804+A2:
1 m2 DuPont™ AirGuard® 5816X
Indicator Unit A1-A3 A4 A5 C4 D
Hazardous waste disposed [kg] 2.24E-9 1.07E-12 1.03E-13 0.00E+0 -8.23E-10
Non-hazardous waste disposed [kg] 2.63E-1 3.19E-5 4.08E-4 0.00E+0 -2.14E-3
Radioactive waste disposed [kg] 8.60E-4 2.76E-7 1.51E-8 0.00E+0 -2.58E-4
Components for re-use [kg] 0.00 0.00 0.00 0.00 0.00
Materials for recycling [kg] 0.00 0.00 0.00 0.00 0.00
Materials for energy recovery [kg] 0.00 0.00 0.00 0.00 0.00
Exported electrical energy [MJ] 0.00E+0 0.00E+0 0.00E+0 1.38E-3 9.05E-1
Exported thermal energy [MJ] 0.00E+0 0.00E+0 0.00E+0 2.49E-3 2.98E+0
RESULTS OF THE LCA – additional impact categories according to EN 15804+A2-optional:
1 m2 DuPont™ AirGuard® 5816X
Indicator Unit A1-A3 A4 A5 C4 D
Potential incidence of disease due to PM emissions [Disease
ND ND ND ND ND
Incidence]
Potential Human exposure efficiency relative to U235 [kBq U235-
ND ND ND ND ND
Eq.]
Potential comparative toxic unit for ecosystems [CTUe] ND ND ND ND ND
Potential comparative toxic unit for humans - cancerogenic [CTUh] ND ND ND ND ND
Potential comparative toxic unit for humans - not cancerogenic [CTUh] ND ND ND ND ND
Potential soil quality index [-] ND ND ND ND ND
Disclaimer 1 – for the indicator “Potential Human exposure efficiency relative to U235”.
This impact category deals mainly with the eventual impact of low dose ionizing
radiation on human health of the nuclear fuel cycle. It does not consider effects due to possible
nuclear accidents, occupational exposure nor due to radioactive waste disposal in underground
facilities. Potential ionizing radiation from the soil, from radon and from some construction materials is also not
measured by this indicator.
Disclaimer 2 – for the indicators “abiotic depletion potential for non-fossil resources”, “abiotic depletion potential
for fossil resources”, “water (user) deprivation potential, deprivation-weighted water consumption”, “potential
comparative toxic unit for ecosystems”, “potential comparative toxic unit for humans – cancerogenic”, “Potential
comparative toxic unit for humans - not cancerogenic”, “potential soil quality index”.
The results of this environmental impact indicator shall be used with care as the
uncertainties on these results are high or as there is limited experienced with the indicator.
References
Standards EN ISO 14025:2011, Environmental labels and
declarations — Type III environmental declarations —
EN 12310-1 Principles and procedures.
EN 12310-1:1999, Flexible sheets for waterproofing -
Part 1: Bitumen sheets for roof waterproofing; Further References
determination of resistance to tearing (nail shank).
BNB
EN 12311-1 Bewertungssystem Nachhaltiges Bauen
EN 12311-1:1999, Flexible sheets for waterproofing - https://www.nachhaltigesbauen.de/austausch/nutzungs
Part 1: Bitumen sheets for roof waterproofing; dauern-von-bauteilen/
Determination of tensile properties
GaBi software and database:2022
EN 13501-1 GaBi software/database, version 10.6.2.9. Sphera
EN 13501-1:2019, Fire classification of construction Solutions GmbH, 2022.
products and building elements - Part 1: Classification
using data from reaction to fire tests IBU 2021
Institut Bauen und Umwelt e.V.: General Instructions
EN 13984 for the EPD programme of Institut Bauen und Umwelt
EN 13984:2013, Flexible sheets for waterproofing - e.V., Version 2.0, Berlin: Institut Bauen und Umwelt
Plastic and rubber vapour control layers - Definitions e.V., 2021. www.ibu-epd.com
and characteristics
PCR 2021, Part A
EN 15804 PCR Guidance-Texts for Building-Related Products
EN 15804:2012+A2:2019+AC:2021, Sustainability of and Services: Calculation Rules for the Life Cycle
construction works — Environmental Product Assessment and Requirements on the Project Report
Declarations — Core rules for the product category of according to EN 15804+A2:2019
construction products.
PCR 2017, Part B
EN 1849-2 PCR Guidance-Texts for Building-Related Products
EN 1849-2:2019, Flexible sheets for waterproofing - and Services: Requirements on the EPD for False
Determination of thickness and mass per unit area - ceiling and underlay sheeting (version 1.6, 2017)
Part 2: Plastic and rubber sheets
DuPont™, the DuPont Oval Logo, and all trademarks
EN 1931 and service marks denoted with ™, SM or ® are
EN 1931:2000, Bitumen, plastic and rubber sheets for owned by affiliates of DuPont de Nemours, Inc. unless
roof waterproofing - Determination of water vapour otherwise noted.
transmission properties
ISO 14025
6 Environmental Product Declaration DuPont de Nemours (s.à.r.l.) – DuPont™ AirGuard® Air & Vapour Control Layers
(5816X)
Publisher
Institut Bauen und Umwelt e.V. Tel +49 (0)30 3087748- 0
Hegelplatz 1 Fax +49 (0)30 3087748- 29
10117 Berlin Mail info@ibu-epd.com
Germany Web www.ibu-epd.com
Programme holder
Institut Bauen und Umwelt e.V. Tel +49 (0)30 - 3087748- 0
Hegelplatz 1 Fax +49 (0)30 – 3087748 - 29
10117 Berlin Mail info@ibu-epd.com
Germany Web www.ibu-epd.com
Author of the Life Cycle
Assessment Tel 00352-275888-1
Luxembourg Institute of Science Fax 00352-275888-555
and Technology (LIST) Mail info@list.lu
Avenue des Hauts-Fourneaux 5 Web www.list.lu
4362 Esch/Alzette
Luxembourg
Owner of the Declaration
DuPont de Nemours (Luxembourg) Tel +352 3666 5210
s.à r.l. Fax +352 3666 0000
Rue Général Patton 1 Mail tyvek.info@dupont.com
2984 Contern Web www.dupont.com
Luxembourg
