ENVIRONMENTAL PRODUCT DECLARATION
as per ISO 14025 and EN 15804+A2
Owner of the Declaration Hansgrohe Group
Publisher Institut Bauen und Umwelt e.V. (IBU)
Programme holder Institut Bauen und Umwelt e.V. (IBU)
Declaration number EPD-HAN-20230026-ICC2-EN
Issue date 24.02.2023
Valid to 23.02.2028
Shower and Bath Faucets
Hansgrohe Group
www.ibu-epd.com | https://epd-online.com
1. General Information
Hansgrohe Group Shower and Bath Faucets
Programme holder Owner of the declaration
IBU – Institut Bauen und Umwelt e.V. Hansgrohe Group
Hegelplatz 1 Auestr. 5-9
10117 Berlin 77761 Schiltach
Germany Germany
Declaration number Declared product / declared unit
EPD-HAN-20230026-ICC2-EN One (1) piece of an average shower and bath faucet incl. packaging
This declaration is based on the product category rules: Scope:
Fittings and showers, 01.08.2021 This average EPD was determined on the basis of a weighted average of
(PCR checked and approved by the SVR) production volume from 2021 and relates to the plants in Offenburg and
Schiltach, Germany, Shanghai, China and Alpharetta, USA. This average
EPD is valid for the whole product group of chrome plated shower and
Issue date bath faucets. The EPD was formed from >95% of the products involved in
the sales quantity.
24.02.2023
The owner of the declaration shall be liable for the underlying information
and evidence; the IBU shall not be liable with respect to manufacturer
information, life cycle assessment data and evidences.
Valid to
23.02.2028 The EPD was created according to the specifications of EN 15804+A2. In
the following, the standard will be simplified as EN 15804.
Verification
The standard EN 15804 serves as the core PCR
Independent verification of the declaration and data according to ISO
14025:2011
internally X externally
Dipl.-Ing. Hans Peters
(Chairman of Institut Bauen und Umwelt e.V.)
Florian Pronold Dr Naeem Adibi,
(Managing Director Institut Bauen und Umwelt e.V.) (Independent verifier)
1 Environmental Product Declaration - Hansgrohe Group - Shower and Bath Faucets
2. Product
products or multiple products with outer packaging. The
2.1 Product description/Product definition products with the smallest and the largest volume have
Shower faucets dimensions between 75x75x215 mm and 380x220x1200 mm.
and bath faucets essentially comprise of a metal housing in
most cases made of brass, 2.5 Base materials/Ancillary materials
a plastic valve with ceramic discs and several assembly parts of The material composition (incl. packaging) of an average
various shower and bath faucet is as follows:
materials. The faucet surface is usually chrome-plated by Name Value Unit
means of various
Brass 54.1 %
galvanic process stages.
Cardboard, Paper 24.0 %
Zinc 9.8 %
Plastic 6.7 %
Polyphenylene 2.0 %
For the use
Stainless steel 1.5 %
and application of the product the respective national provisions
Other material 1.0 %
at the place
of use apply, in Germany for example the building codes of the Other metals 0.9 %
federal states The parts which are made of brass contain between 0.2 and
and the corresponding national specifications. 1.4% lead.
The products comply with This product contains substances listed in the candidate list
the applicable standards and regulations listed below. Following (date: 17.12.2021) exceeding 0.1 percentage by mass: Lead
standards depending on the operating mechanism may apply to (CAS number 7439-92-1) as a component of the brass alloy
shower and bath faucets to prove product safety: has been on the candidate list of the Reach Regulation
• EN 817:2008: Sanitary tapware – Mechanical mixing (Regulation (EC) No. 1907/2006) since 27.06.2018.
valves (PN 10)
• EN 200:2008: Sanitary tapware – Single taps and This product/article/at least one partial article contains other
combination taps for water supply systems of type 1 and CMR substances in categories 1A or 1B which are not on the
type 2 candidate list, exceeding 0.1 percentage by mass: no.
• ISO 3822: Acoustics – Laboratory tests on noise
emission from appliances and equipment used in water Biocide products were added to this construction product or it
supply installations has been treated with biocide products (this then concerns a
treated product as defined by the (EU) Ordinance on Biocide
2.2 Application Products No. 528/2012): no.
Shower and bath faucets are plumbing fixtures that mix hot and
2.6 Manufacture
cold water, shut off water,
and regulate the amount of water. They are mechanically
operated by handles and
are used in showers and bathtubs.
2.3 Technical Data
The
products must comply with the standard DIN EN 1113 and
specific Hansgrohe
standards.
Constructional data
Name Value Unit
Maximum load temperature
65 °C
permanent operation
Maximum load temperature
90 °C
temporary operation
Flow rate (indications for Depending on the
m3/h
pressure range of 1-3 bar) product 0,09 to 1,2
Sound emissions < 30 dB
Performance
data of the product with respect to its characteristics in
No. 1: The
accordance with the
sand core for the base body is made.
relevant technical provision (no CE-marking).
2.4 Delivery status
The shower and bath faucets are delivered singularly
No. 2: The
packaged. The packaging is
body of the faucet is cast from brass using the sand core.
customized to the size of the product and supplies. Customers
can order single
2 Environmental Product Declaration - Hansgrohe Group - Shower and Bath Faucets
No. 3: In addition, all production sites are certified according to the
After casting, the brass body is grinded and polished. DIN EN
ISO standards 14001 (environment), 50001 (energy), 45001 (occupational
health and safety) and 9001 (quality). Continuous improvement
of environmental and occupational safety performance is thus
No. 4: To protect guaranteed.
the product and make it durable, the body is galvanized with
chrome. 2.8 Product processing/Installation
Installation
of exposed faucets
The
No. 5: protective caps are removed and transitions from the
Meanwhile, the individual parts of the cartridge are assembled. connections to the tiles
are sealed with the fingers (tools: water, washing-up liquid).
No. 6: The
product parts (chrome plated brass body, cartridge, chrome The S-connectors
plated handle and are adjusted to installation length (tool: hand saw).
others) are lasered and assembled.
Next, the
No. 7: The S-connectors are screwed in, sealed and aligned (tools:
preassembled product is packed together with the remaining wrench, spirit level).
components (like s-connectors
and escutcheon).
The escutcheons
are screwed over the S-connectors.
Any production waste generated is disposed accordingly. In
individual cases, the production may differ slightly from the
procedure (for
example, if the brass body is purchased and not manufactured Then the
in-house). fitting is screwed on (tool: wrench).
2.7 Environment and health during manufacturing
Hansgrohe SE tries to keep the
impact on people and the environment as low as possible when The handle
manufacturing its is removed to adjust the temperature setting of the cartridge
products. and to adjust the
Hazards at workplaces are regularly anti-scald protection (tools: standard hexagonal offset
assessed and reduced to a minimum. screwdriver and
pliers).
For example, in basic production,
sawing or grinding work is mainly carried out by robots, and in The handle
electroplating, is then reattached (tool: standard hexagonal offset screwdriver).
chemicals are dosed automatically via appropriate pump
stations.
Emissions that are hazardous to
health are extracted directly at the source and cleaned by filter
systems. Installation
of concealed faucets
Workplace and emission limits are
regularly monitored and are far below the prescribed limits. The housing
of the basic set is cut to length (tool: cutter knife). The
protective cap and
rinsing block are removed (tool: hexagonal offset screwdriver).
To reduce environmental impact,
water and production waste are recycled wherever possible.
3 Environmental Product Declaration - Hansgrohe Group - Shower and Bath Faucets
The basic The quality and durability of our shower and bath faucets is
set is then sealed again with a silicone joint (tools: silicone designed for a product life of about 20 years. Which on average
syringe, is approximately
fingers, water, washing-up liquid). the function block is put on the duration of use by the consumers. With few exceptions, all
(tool: hexagonal products have a five-year warranty. Furthermore, an after-sale
offset screwdriver). Then the plastic screws for the rosette service warranty of 15 years is provided.
holder are cut to
length and screwed on (tools: handsaw and screwdriver). 2.13 Extraordinary effects
Fire
The
products are not classified as building materials (building
Optional: products) and are
the joints under the visible escutcheon can be sealed with not subject to DIN 4102 and EN 13501-1.
silicone (tools:
Fire protection
silicone syringe, fingers, water, washing-up liquid). The visible
Name Value
escutcheon is
applied to the functions (diverter, mixer, etc.). The visible Building material class
escutcheon is Burning droplets
pressed on (tool: hexagonal offset screwdriver). Smoke gas development
Water
If a room in which the products
The
offered by Hansgrohe are installed is flooded with water, the
temperature of the cartridge must be set and the anti-scald
electronic
protection had to
faucets may be destroyed. All other products are not affected in
be adjusted (tools: standard hexagonal offset screwdriver and
their
pliers).
function.
There will be no environmental
The handle
impact.
is then attached (tool: standard hexagonal offset screwdriver).
2.9 Packaging Mechanical destruction
For product If the surface of the coating is
protection the shower faucets and bath faucets are individually destroyed by a mechanical stress, there is a possibility of
packed in a corrosion.
cardboard box, which consists of approximately 80% recycled In the event of mechanical
material. The damage, the products may need to be replaced due to possible
cardboard is always printed with lead-free ink and in some sharp cut edges.
cases additionally
2.14 Re-use phase
coated with clear topcoat. The inlay of the packaging consists
The shower
of folded cardboard,
and bath faucets are not taken back by the manufacturer for the
fiber form or plastic bags, depending on the product.
purpose of
The
reuse. Users can disassemble the products repeatedly within
packaging can be fully recycled.
the reference utilization
period and reuse it elsewhere.
2.15 Disposal
All
The waste code of the product is
packaged products fit on a reusable euro pallet.
AVV 20 03 01. Disassembly of
2.10 Condition of use the products consists of the same steps as assembly, in
reverse order.
To protect
the shower and bath faucets and make them durable, the body
and handle are made
All metal
of chrome-plated metal. Nevertheless, there are no unhealthy
components can be recycled (as scrap).
contaminants in
All plastic components have a high calorific value and can be
the water. To ensure the longevity of the product, it should be
sent for thermal recycling.
used and
In countries where no thermal recycling or substance recycling
cleaned regularly.
is established, disposal takes place via the waste incineration
2.11 Environment and health during use plant.
Our products do not emission any contaminants or substances
2.16 Further information
that are
Additional
harmful to the environment or health during the use phase.
information about our products can be found at
2.12 Reference service life https://www.hansgrohe.com.
3. LCA: Calculation rules
4 Environmental Product Declaration - Hansgrohe Group - Shower and Bath Faucets
3.1 Declared Unit
The results of Maintenance
this EPD are valid for the following functional unit: expenses are declared in this module and consist of weekly
cleaning expenses and cartridge replacement.
Provide
sanitary function for one (1) average shower and bath faucet
unit used in accordance with
the manufacturer's recommendations for a 20-year life, Modules C1-C4:
following the The modules include the environmental impacts for dismantling
manufacturer's operating instructions. An average conditioned of the products and the treatment of the waste fractions until
shower and bath faucet is considered the baseline flow. the end-of-waste status (EoW) is reached, including the
associated transports at the end of the product life cycle.
Module D:
Identification
Weighted averaging based on production tonnages in of the benefits and costs of the product outside the system
2021 is chosen as basis for creating the environmental profile. boundary. For waste,
163 different shower and bath faucets were considered. paper and plastics, these consist of energy credits from thermal
Functional unit utilization (A3,
A5 and C3) in the form of the average European electricity mix
Name Value Unit
or thermal energy
Declared unit 1 pce.
from natural gas. Recycling of paper, plastic and metal scrap
Functional unit 1 pce. results in
Functional unit with packaging 2.36 kg credits of the respective raw materials for the primary material
Packaging 0.60 kg portion of the input. The loads of the waste incineration and
recycling processes are assigned to the respective modules
Weight range of the products examined 0.49 - 13.83 kg
(A3, A5 and C3) and
Other declared units are allowed if the conversion is shown not to module D.
transparently.
3.3 Estimates and assumptions
For IBU core EPDs (where clause 3.6 is part of the EPD): for Energy and water consumption, material amount for coating as
average EPDs, an estimate of the robustness of the LCA well as waste during production could only be determined on
values must be made, e.g. concerning the variability of the concrete, existing products and not on the average product.
production process, geographical representativeness and the The highest value of all inputs and outputs for energy, waste
influence of background data and preliminary products and coating of the top seller, the lightest and the heaviest
compared to the environmental impacts caused by the actual product was used for the calculation of energy, water, waste
production. and coating. For the incineration with energy recovery (thermal
and electric) of waste, an r1 value of > 0.6 is assumed. The net
efficiency for the average waste incinerated is between 38 %
3.2 System boundary
and 44 %, depending on the type of waste respectively the
This representative EPD follows the EPD type "cradle to gate - disposal data set.
with options". The following life cycle modules are declared:
Modules A1-A3: 3.4 Cut-off criteria
The product stage begins with considering the production of the The effect associated with the neglected mass
necessary raw materials and energies, including all shares is less than 5% of the effect categories per module. The
corresponding upstream chains and the actual procurement minimum limit
transports. Furthermore, the entire manufacturing phase was of 1% total mass and the use of renewable and nonrenewable
mapped, including the treatment of production waste until the primary energy is
end-of-waste status (EoW) was reached. Green electricity from not exceeded.
hydropower is used for the manufacturing processes in
Germany. US electricity mix is used for the US production site. 3.5 Background data
Chinese electricity mix is used for the Chinese production site, The LCA software GaBi 10.6 was used to model the life cycle.
although electricity from photovoltaic is partly used there. The entire manufacturing process, as well as energy
consumption, were modelled on the basis of manufacturer
Module A4: specific data.
All distribution transports to the customers were considered. However, generic background datasets were used for the
Module A5: upstream and downstream processes. The majority of the
This module covers the installation process with the background datasets used were taken from the current version
corresponding packaging waste generated that needs to be (2021.2) of the GaBi database. Ecoinvent Version 3.6 (2019)
disposed. datasets were only used when suitable GaBi datasets were not
available.
Modules B1 & B3-B7:
3.6 Data quality
These modules were considered, but evaluated as not relevant
for the products and considered as zero. The background datasets used for accounting purposes mainly
originate from the respective updated GaBi databases at the
Module B2: time of calculation. The data for the examined products was
5 Environmental Product Declaration - Hansgrohe Group - Shower and Bath Faucets
captured on metallurgical waste in C3 are credited in module D.
the basis of evaluations of internal production and Credits
environmental data, the collection of LCA relevant data within for the energy recovery of incinerated production waste in A1-3,
the supply chain, as well as the evaluation of relevant data for paper,
the energy supply. The collected cardboard and plastics in A5 and plastics and other materials in
data were checked for plausibility and consistency. Good C3 are
representativity can be assumed. credited in module D.
The loads for
For the assessment of the variability of the results, all products waste water treatment and waste disposal of core sand, waste
were balanced in addition to the average product. See at oil and
chapter 6 for explanation of the variability. hazardous waste from the manufacturing phase are allocated
to module A3.
3.7 Period under review
Life cycle assessment data were collected in Packaging:
2021. For
paper and cardboard, recycling (91 %) and energy recovery (9
3.8 Geographic Representativeness
%) are
Land or region, in which the declared product system is considered on a pro rata basis. For plastic, a proportionate
manufactured, used or handled at the end of the product´s recycling
lifespan: Global (52 %), energy recovery (48 %) considered, based on Eurostat.
Deconstructed product at the end of life:
Since
3.9 Allocation
the product is predominantly made of
For the production process nearly all raw materials, precursors
metal, it is assumed that most of its metallic components are
and supplies could be assigned to the declared product.
recycled.
Energy, water,
95 % of the non-metallic components are incinerated with
galvanization process and production waste were assigned to
energy recovery
the highest
and 5 % are disposed in landfill. For the metal components, it is
value of either the heaviest, lightest or most sold product of the
assumed that 90 % are sent for material recycling, 5 % for
product group. No byproducts are produced and no allocation is
incineration
required.
with energy recovery (C3) and 5 % are disposed in landfill (C4).
Some
of the brass losses from brass processing in module A3 are 3.10 Comparability
directly
Basically, a comparison or an evaluation of EPD data is only
reused by Hansgrohe and are modelled as a closed loop.
possible if all the data sets to be compared were created
Another part of
according to EN 15804 and the building context, respectively
the brass losses (brass particles and dusts) is disposed of as
the product-specific characteristics of performance, are taken
waste
into account.
(without debits and credits).
The used background database has to be mentioned.
Credits for plastics, paper and cardboard recycled in A5 and
4. LCA: Scenarios and additional technical information
Transport to the building site (A4)
Characteristic product properties of biogenic carbon
The biogenic carbon content quantifies the amount of biogenic Name ValueUnit
carbon in a construction product leaving the factory gate, and it Transport distance (Truck) 439 km
shall be separately declared for the product and for any Capacity utilisation (including empty runs) (Truck) 55 %
accompanying packaging.
Transport distance (Container Ship) 6871 km
If the total mass of biogenic carbon containing materials is less
Capacity utilisation (Container Ship) 80 %
than 5 % of the total mass of the product and accompanying
packaging, the declaration of biogenic carbon content may be
Installation into the building (A5)
omitted. The mass of packaging containing biogenic carbon
For the installation are required silicone and teflon tape. The
shall always be declared.
packaging is disposed either by recycling or incineration.
Name Value Unit
Information on describing the biogenic Carbon Content at
Packaging waste (Paper, cardboard, plastic) 0.603 kg
factory gate
Silicone 0.02 kg
The biogenic carbon content was calculated based on the
factors from the Teflon tape 0.1 m
Thünen Intitute.
Maintenance (B2)
Name ValueUnit
For
Biogenic carbon content in accompanying kg
0.23 module B2, it is assumed that a weekly cleaning of the product
packaging C
takes place,
Note: 1 kg of biogenic carbon is equivalent to 44/12 kg of CO . with 0.5 liter of water containing 1.5% soap.
2
The cartridge is
replaced once during its service life.
The following technical information is a basis for the declared
modules
6 Environmental Product Declaration - Hansgrohe Group - Shower and Bath Faucets
Name Value Unit and bath faucets when used
in accordance with the care instructions. This value is based on
Maintenance cycle (cleaning) 1040 Number/RSL
their
Water consumption/Cycle weekly
0.5 Liter/cycle technical service centre's statistics on service life in the market
(cleaning)
and
Soap concentration (cleaning) 1.5 %
complaints.
Water consumption (cleaning) 0.52 m3
Name Value Unit
Auxiliary Soap/Tensides (cleaning) 7.8 kg Life Span according to the manufacturer 20 a
Maintenance Cycle (cartridge
1 Number/RSL
replacement) End of life (C1-C4)
Cartridge (cartridge replacement) 0.0581 kg/RSL Name Value Unit
Collected separately waste type 1.761 kg
In case a reference service life according to applicable ISO Recycling 1.424 kg
standards is declared then the assumptions and in-use Energy recovery 0.249 kg
conditions underlying the determined RSL shall be declared. In Landfilling 0.088 kg
addition, it shall be stated that the RSL applies to the reference
conditions only.
Reuse, recovery and/or recycling potentials (D), relevant
The same holds for a service life declared by the manufacturer. scenario information
Corresponding information related to in-use conditions needs The
not be provided if a service life taken from the list of service life energy generated from energy recovery as well as recycled
by BNB is declared. materials are
assigned to module D as possible potentials or avoided loads in
subsequent systems. Credits are only given for the primary
Service life
portion of
Hansgrohe SE declares
the inputs.
a Service Life of 20 years as an empirical value for the shower
7 Environmental Product Declaration - Hansgrohe Group - Shower and Bath Faucets
5. LCA: Results
The following table shows the result of the LCA
for 1 piece of an average shower and bath faucet. The results in the B-module are based on
a lifetime of 20 years.
DESCRIPTION OF THE SYSTEM BOUNDARY (X = INCLUDED IN LCA; MND = MODULE OR INDICATOR NOT DECLARED; MNR
= MODULE NOT RELEVANT)
Benefits and
Construction loads beyond
Product stage Use stage End of life stage
process stage the system
boundaries
la ire ta m w a Ry lp p u s tro p s n a rT g n iru tc a fu n a M e h t m o rf tro p s n a rTe tis e h t o t e ta g y lb m e s s A e s U e c n a n e tn ia M ria p e R tn e m e c a lp e R tn e m h s ib ru fe R y g re n e la n o ita re p Oe s u re ta w la n o ita re p Oe s u n o itc u rts n o c -e Dn o itilo m e d tro p s n a rT g n is s e c o rp e ts a W la s o p s iD -e s u e R-y re v o c e R-g n ilc y c e Rla itn e to p
A1 A2 A3 A4 A5 B1 B2 B3 B4 B5 B6 B7 C1 C2 C3 C4 D
X X X X X X X X X X X X X X X X X
RESULTS OF THE LCA - ENVIRONMENTAL IMPACT according to EN 15804+A2: 1 piece average shower and bath faucet incl.
packaging
Parameter Unit A1-A3 A4 A5 B1 B2 B3 B4 B5 B6 B7 C1 C2 C3 C4 D
-4.06E
GWP-total kg CO 2 eq 5.82E+00 2.25E-01 1.07E+00 0 2.59E+01 0 0 0 0 0 0 3E-02 3.89E-01 4.51E-03 +00
-3.23E
GWP-fossil kg CO 2 eq 6.63E+00 2.24E-01 2.36E-01 0 1.99E+01 0 0 0 0 0 0 2.98E-02 3.89E-01 4.51E-03 +00
GWP-
biogenic kg CO 2 eq -8.29E-01 0 8.29E-01 0 0 0 0 0 0 0 0 0 0 0 -8.17E-01
GWP-luluc kg CO 2 eq 1.71E-02 7.24E-04 3.12E-04 0 6.02E+00 0 0 0 0 0 0 2.44E-04 8.32E-05 4.38E-06 -1E-02
kg CFC11
ODP 9.54E-09 3.15E-17 1.46E-15 0 1.09E-06 0 0 0 0 0 0 5.9E-18 7.23E-11 1.06E-17 -1.09E-08
eq
AP mol H+ eq 7.34E-02 5.16E-03 5.4E-04 0 6.7E-02 0 0 0 0 0 0 4.99E-05 1.89E-04 1.42E-05 -3.93E-02
EP-
kg P eq 4.56E-05 2.93E-07 3.79E-07 0 5.81E-04 0 0 0 0 0 0 8.88E-08 1.35E-07 1.21E-07 -1.26E-05
freshwater
EP-marine kg N eq 8.61E-03 1.38E-03 1.27E-04 0 1.53E-02 0 0 0 0 0 0 1.97E-05 7.68E-05 3.65E-06 -4.14E-03
EP-terrestrial mol N eq 9.11E-02 1.52E-02 1.41E-03 0 1.82E-01 0 0 0 0 0 0 2.25E-04 8.98E-04 3.86E-05 -4.39E-02
kg
POCP NMVOC 2.55E-02 3.84E-03 4.23E-04 0 6.08E-02 0 0 0 0 0 0 4.46E-05 1.99E-04 1.14E-05 -1.25E-02
eq
ADPE kg Sb eq 3.15E-03 1.19E-08 2.81E-06 0 2.2E-05 0 0 0 0 0 0 2.65E-09 1.3E-08 3.07E-10 -2.3E-03
-3.76E
ADPF MJ 8.88E+01 2.83E+002.74E+00 0 4.56E+02 0 0 0 0 0 0 3.98E-01 5.13E-01 6.48E-02
+01
m3 world
-7.13E
WDP eq 9.99E+00 1.03E-03 6.21E-02 0 6.96E+00 0 0 0 0 0 0 2.77E-04 4.13E-02 -4.83E-05
+00
deprived
GWP = Global warming potential; ODP = Depletion potential of the stratospheric ozone layer; AP = Acidification potential of land and water; EP =
Eutrophication potential; POCP = Formation potential of tropospheric ozone photochemical oxidants; ADPE = Abiotic depletion potential for non-fossil
resources; ADPF = Abiotic depletion potential for fossil resources; WDP = Water (user) deprivation potential)
RESULTS OF THE LCA - INDICATORS TO DESCRIBE RESOURCE USE according to EN 15804+A2: 1 piece average shower
and bath faucet incl. packaging
Parameter Unit A1-A3 A4 A5 B1 B2 B3 B4 B5 B6 B7 C1 C2 C3 C4 D
-1.19E
PERE MJ 2.08E+01 7.33E-02 1.05E+01 0 9.4E+01 0 0 0 0 0 0 2.29E-02 2.6E-01 4.69E-03
+01
-9.34E
PERM MJ 9.34E+00 0 0 0 0 0 0 0 0 0 0 0 0 0
+00
-1.19E
PERT MJ 3.01E+01 7.33E-02 1.18E+00 0 9.4E+01 0 0 0 0 0 0 2.29E-02 2.6E-01 4.69E-03
+01
-3.77E
PENRE MJ 8.16E+012.83E+00 4.5E+00 0 4.56E+02 0 0 0 0 0 0 4E-01 5.79E+00 3.43E-01
+01
-1.76E -5.28E
PENRM MJ 7.32E+00 0 0 0 0 0 0 0 0 0 0 -2.78E-01 0
+00 +00
-3.77E
PENRT MJ 8.89E+012.83E+002.74E+00 0 4.56E+02 0 0 0 0 0 0 4E-01 5.13E-01 6.48E-02
+01
SM kg 1.14E+00 0 0 0 2.46E-03 0 0 0 0 0 0 0 0 0 1.03E+00
RSF MJ 7.1E-24 0 0 0 0 0 0 0 0 0 0 0 0 0 -2.1E-23
NRSF MJ 0 0 0 0 0 0 0 0 0 0 0 0 0 0 0
FW m3 2.34E-01 8.67E-05 2.03E-03 0 1.63E-01 0 0 0 0 0 0 2.62E-05 1.07E-03 7.75E-07 -1.6E-01
PERE = Use of renewable primary energy excluding renewable primary energy resources used as raw materials; PERM = Use of renewable primary
energy resources used as raw materials; PERT = Total use of renewable primary energy resources; PENRE = Use of non-renewable primary energy
excluding non-renewable primary energy resources used as raw materials; PENRM = Use of non-renewable primary energy resources used as raw
8 Environmental Product Declaration - Hansgrohe Group - Shower and Bath Faucets
materials; PENRT = Total use of non-renewable primary energy resources; SM = Use of secondary material; RSF = Use of renewable secondary fuels;
NRSF = Use of non-renewable secondary fuels; FW = Use of net fresh water
RESULTS OF THE LCA – WASTE CATEGORIES AND OUTPUT FLOWS according to EN 15804+A2:
1 piece average shower and bath faucet incl. packaging
Parameter Unit A1-A3 A4 A5 B1 B2 B3 B4 B5 B6 B7 C1 C2 C3 C4 D
HWD kg 1.48E-06 7.5E-11 2.37E-09 0 8.5E-03 0 0 0 0 0 0 2.11E-11 1.57E-10 1.15E-11 -8.06E-06
NHWD kg 1.27E+00 3.51E-04 3.68E-02 0 6.97E-01 0 0 0 0 0 0 6.27E-05 2.68E-02 8.8E-02 -8.54E-01
RWD kg 2.87E-03 3.98E-06 1.34E-04 0 4.21E-03 0 0 0 0 0 0 7.25E-07 3.5E-05 7.4E-07 -1.64E-03
CRU kg 0 0 0 0 0 0 0 0 0 0 0 0 0 0 0
MFR kg 0 0 5.29E-01 0 0 0 0 0 0 0 0 0 1.42E+00 0 0
MER kg 0 0 0 0 9.01E-04 0 0 0 0 0 0 0 0 0 0
EEE MJ 2.11E-01 0 2.39E-01 0 1.58E-01 0 0 0 0 0 0 0 2.89E-02 2.9E-04 0
EET MJ 6.18E-01 0 4.29E-01 0 2.87E-01 0 0 0 0 0 0 0 5.42E-02 0 0
HWD = Hazardous waste disposed; NHWD = Non-hazardous waste disposed; RWD = Radioactive waste disposed; CRU = Components for re-use;
MFR = Materials for recycling; MER = Materials for energy recovery; EEE = Exported electrical energy; EET = Exported thermal energy
RESULTS OF THE LCA – additional impact categories according to EN 15804+A2-optional:
1 piece average shower and bath faucet incl. packaging
Parameter Unit A1-A3 A4 A5 B1 B2 B3 B4 B5 B6 B7 C1 C2 C3 C4 D
Disease
PM 6.91E-07 8.67E-08 5.62E-09 0 3.32E-06 0 0 0 0 0 0 3.12E-10 1.21E-09 1.52E-10 -3.67E-07
incidence
kBq U235
IR 1.28E+00 5.75E-04 2.11E-02 0 2.15E+00 0 0 0 0 0 0 1.06E-04 3.38E-03 1.06E-04 -9.98E-01
eq
-3.27E
ETP-fw CTUe 2.62E+022.07E+001.02E+00 0 2.02E+02 0 0 0 0 0 0 2.95E-01 3.09E-01 2.5E-02
+01
HTP-c CTUh 4.86E-08 3.99E-11 7.39E-10 0 2.71E-08 0 0 0 0 0 0 5.98E-12 1.02E-11 2.3E-12 -6.86E-09
HTP-nc CTUh 4.72E-07 1.98E-09 8.47E-08 0 7.56E-07 0 0 0 0 0 0 3.18E-10 6.89E-10 2.26E-10 -2.58E-07
-3.25E
SQP SQP 6.17E+01 4.08E-01 4.74E+00 0 3.18E+02 0 0 0 0 0 0 1.37E-01 2.13E-01 4.75E-03
+01
PM = Potential incidence of disease due to PM emissions; IR = Potential Human exposure efficiency relative to U235; ETP-fw = Potential comparative
Toxic Unit for ecosystems; HTP-c = Potential comparative Toxic Unit for humans (cancerogenic); HTP-nc = Potential comparative Toxic Unit for humans
(not cancerogenic); SQP = Potential soil quality index
Disclaimer 1 – for the indicator “Potential Human exposure efficiency relative to U235”. This impact category deals mainly with the
eventual impact of low-dose ionizing radiation on human health of the nuclear fuel cycle. It does not consider effects due to possible
nuclear accidents, occupational exposure or radioactive waste disposal in underground facilities. Potential ionizing radiation from the
soil, radon and from some construction materials is also not measured by this indicator.
Disclaimer 2 – for the indicators “abiotic depletion potential for non-fossil resources”, “abiotic depletion potential for fossil resources”,
“water (user) deprivation potential, deprivation-weighted water consumption”, “potential comparative toxic unit for ecosystems”,
“potential comparative toxic unit for humans – cancerogenic”, “Potential comparative toxic unit for humans - not cancerogenic”,
“potential soil quality index”. The results of this environmental impact indicator shall be used with care as the uncertainties on these
results are high as there is limited experience with the indicator.
6. LCA: Interpretation
9 Environmental Product Declaration - Hansgrohe Group - Shower and Bath Faucets
materials.
The dominance analysis shows that module
B2 in particular is the dominant life cycle stage in most
indicators, due to
the demand of soap and water for cleaning. The module A1-A3 1,252,324 bath and shower faucets of
has the second most 163 different product types were produced. For the assessment
input regarding GWP total (5.82 kg CO2-eq.). This is mainly of the
caused variability of the results, all products were balanced and
by the provision of brass for the production of the bath and compared to the
shower faucets at average product weighted by production volume.
the production site (3.49 kg CO2-eq.)
The different types of products all
ADPE differs from the other have the same function and differ mainly in terms of design,
indicators. The provision of brass in A1-A3 has the largest which has an
contribution. influence on construction and materials used. The basic
structure of the
product types is always similar. Material type and quantity
proportions do not
The end-of-life stage has no differ much, as also shown in the average material composition
significant influence on the environmental indicators. table.
The environmental burdens from the The deviation of the GWP fossil in
transport (module A4) have a low but noticeable impact on AP, modules A1-C4 has a maximum of 91% and a minimum of -
EPmarine, 22%. 55% of the bath and
EPterrestrial and POCP. shower faucets produced are above the average GWP fossil
value and 45% reflect
the average or are lower than the average. However, 91% of
the ones which are
The possible potentials of avoided above the average just deviate between +1 and +11 %.
loads of subsequent systems (module D) lie outside the
considered system
boundaries and relate exclusively to credits from recycling and The
thermal deviations in the life cycle results are largely due to the product
recycling by means of incineration with energy recovery of the weight
different (between 0.5 and 13.8 kg). Further reasons are the origin of the
10 Environmental Product Declaration - Hansgrohe Group - Shower and Bath Faucets
brass (brass The products
from China was modelled with a lower recycling content than with a higher plastic content cause a higher GWP impact in the
brass from Germany) end of life
and/or the proportion of plastic, as these vary by product type. because they are incinerated instead of recycled.
7. Requisite evidence
The drinking water regulation determines the quality of drinking • Thermoplastic elastomers: Recommendation for the
water at the point of withdrawal. This result in requirements for hygienic assessment of products made of thermoplastic
used materials in drinking water installations in general and elastomers in contact with drinking water (TPE transition
therefore in sanitary fittings in particular. recommendation)
All materials used by Hansgrohe SE, which are in contact with • Ceramics: draft assessment basis for enamels and
drinking water, fulfill the drinking water regulation. ceramic materials: assessment basis for enamels and
Regulations for metals (Europe-wide): ceramic materials in contact with drinking water
(enamel/ceramic assessment basis)
• Acceptance of metallic materials used for products in
• Lubricants: Guideline for the hygienic assessment of
contact with drinking water: 4MS Common Approach
lubricants in contact with drinking water (sanitary
- Part A – Procedure for the acceptance
lubricants), (Lubricant Guideline)
- Part B – 4MS Common Composition List
Regulation for other materials (France):
• Metal recommendation of the federal environment
• ACS: Attestation de Conformité Sanitaire (plastics,
agency: metal materials suitable for drinking water
elastomers, metals)
hygiene
Regulation for other materials (UK):
Regulations for other materials (Germany):
• BS 69 20: Suitability of non-metallic products for use in
• KTW: Assessment basis for plastics and other organic
contact with water intended for human consumption with
materials in contact with drinking water
regard to their effect on the quality of water (plastics,
• Elastomer guideline: Guideline for the hygienic
elastomers)
assessment of elastomers in contact with drinking water
Products of the Hansgrohe SE are therefore uncritical to use
with any drinking water.
8. References
Standards
DIN EN ISO 14025
DIN EN ISO 14025: Environmental labels and declarations -
EN 200 Type III environmental declarations - Principles and procedures,
EN 200:2008: Sanitary tapware – Single taps and combination 2011-10
taps for water supply systems of type 1 and type 2 EN 15804
EN 817 DIN EN 15804:2012+A2:2019+AC:2021: Sustainability of
EN 817:2008: Sanitary tapware – Mechanical mixing valves construction works - Environmental product declarations - Core
(PN 10) rules for the product category of construction products
ISO 3822 DIN EN ISO 45001
ISO 3822: Acoustics – Laboratory tests on noise emission from DIN EN ISO 45001:2018: Occupational health and safety
appliances and equipment used in water supply installations management systems — Requirements with guidance for use.
2018-03
DIN 4102-1
DIN 4102-1: Fire behaviour of building materials and building DIN EN ISO 50001
components - Part 1: Building materials; concepts, DIN EN ISO 50001:2018: Energy management systems —
requirements and tests. 1998-05 Requirements with guidance for use. 2018-08
Further References
DIN EN ISO 9001
DIN EN ISO 9001:2015: Quality management systems - AVV
Requirements (ISO 9001:2015) Draft General administrative provision relating to the Order on
the European list of wastes (Waste List Order – German
designation: AVV) of 10 December 2001.
DIN EN 13501-1
DIN EN 13501-1:2019-05: Fire classification of construction
products and building elements - Part 1: Classification using ECHA
data from reaction to fire tests; German version EN 13501- European Chemicals Agency (ECHA) Candidate List of
1:2018 Substances of Very High Concern (SVHC) for Authorisation
https://echa.europa.eu/de/candidate-listtable
DIN EN ISO 14001
DIN EN ISO 14001:2015, Environmental management systems Ecoinvent
— Requirements with guidance for use, 2015-09 ecoinvent 3.6 Database on Life Cycle Inventories (Life Cycle
Inventory data), ecoinvent Association, Zürich, 2020
11 Environmental Product Declaration - Hansgrohe Group - Shower and Bath Faucets
Umwelt e.V.
Version 2.0, Berlin: Institut Bauen und Umwelt e.V., 2021,
EU Ordinance on biocide Products No. 528/2012 www.ibu-epd.com
European Parliament, 2012. Regulation (EU) no 528/2012 of
the European parliament and of the council of 22 May 2012
concerning the making available on the market and use of PCR Part A
biocidal products Institut
Bauen und Umwelt e.V. (IBU), Product Category Rules for
Building-Related Products and Services. Part A: Calculation
rules for
the life cycle assessment and requirements on the project
report.
Eurostat Version 2.1, Berlin, 11/2021
PCR Part B
Eurostat, last update 26/10/2021 on Institut Bauen und Umwelt e.V. (IBU), Requirements on the
https://ec.europa.eu/eurostat/databrowser/view/ten00063/default/table?EPD for fittings and showers. Version 1.1, Berlin, 03/2022
ang=en
Thünen Institute
Diestel, Sylvia / Weimar, Holger: Der Kohlenstoffgehalt in
GaBi Holz- und Papierprodukten - Herleitung und
GaBi Umrechnungsfaktoren. Thünen
10.6, GaBi Software System and Database for Life Cycle Working Paper 38. Johann Heinrich von Thünen-Institut.
Engineering version 2021.2, Sphera Solutions GmbH, Hamburg, 2014
Leinfelden-Echterdingen, 1992-2021 The literature referred to in the Environmental Product
Declaration must be listed in full.Standards already fully quoted
in the EPD do not need to be listed here again.
IBU 2021 The current version of PCR Part A and PCR Part B of the PCR
General document on which they are based must be referenced.
Instructions for the EPD programme of Institut Bauen und
12 Environmental Product Declaration - Hansgrohe Group - Shower and Bath Faucets
Publisher
Institut Bauen und Umwelt e.V. +49 (0)30 3087748- 0
Hegelplatz 1 info@ibu-epd.com
10117 Berlin www.ibu-epd.com
Germany
Programme holder
Institut Bauen und Umwelt e.V. +49 (0)30 3087748- 0
Hegelplatz 1 info@ibu-epd.com
10117 Berlin www.ibu-epd.com
Germany
Author of the Life Cycle Assessment
brands & values GmbH +49 421 70 90 84 33
Altenwall 14 info@brandsandvalues.com
28195 Bremen www.brandsandvalues.com
Germany
Owner of the Declaration
Hansgrohe Group +49 7836 51-0
Auestr. 5-9 info@hansgrohe-group.com
77761 Schiltach www.hansgrohe-group.com
Germany
13 Environmental Product Declaration - Hansgrohe Group - Shower and Bath Faucets
