ENVIRONMENTAL PRODUCT DECLARATION
as per ISO 14025 and EN 15804+A2
Owner of the Declaration Hansgrohe Group
Programme holder Institut Bauen und Umwelt e.V. (IBU)
Publisher Institut Bauen und Umwelt e.V. (IBU)
Declaration number EPD-HAN-20210262-ICC1-EN
Issue date 12.09.2022
Valid to 11.09.2027
Shower hoses
Hansgrohe Group
www.ibu-epd.com | https://epd-online.com
Umwelt Produktdeklaration Name des Herstellers – Name des Produkts
1. General Information
Hansgrohe Group Shower hoses
Programme holder Owner of the declaration
IBU – Institut Bauen und Umwelt e.V. Hansgrohe Group
Hegelplatz 1 Auestraße 5 - 9
10117 Berlin 77761 Schiltach
Germany Germany
Declaration number Declared product / declared unit
EPD-HAN-20210262-ICC1-EN 1 piece of an average shower hose incl. packaging
This declaration is based on the product Scope:
category rules: This average EPD was determined on the basis of
Fittings and showers, 03.2022 sales volumes from the year 2020. The shower hoses
(PCR checked and approved by the SVR) are manufactured at the production sites in Willstätt
and Schiltach, Germany and in Atlanta, USA. This
average EPD was formed from >90% of the products
Issue date
involved in sales.
12.09.2022
Valid to
The owner of the declaration shall be liable for the
11.09.2027
underlying information and evidence; the IBU shall not
be liable with respect to manufacturer information, life
cycle assessment data and evidences.
The EPD was created according to the specifications
of EN 15804+A2. In the following, the standard will be
simplified as EN 15804.
Verification
The standard EN 15804 serves as the core PCR
Independent verification of the declaration and data
according to ISO 14025:2011
Dipl. Ing. Hans Peters internally x externally
(chairman of Institut Bauen und Umwelt e.V.)
Dr. Alexander Röder Dr Naeem Adibi
(Managing Director Institut Bauen und Umwelt e.V.)) (Independent verifier)
2. Product
2.1 Product description/Product definition 2.3 Technical Data
Shower hoses essentially comprise of a plastic hose
and metal connectors, made of brass or stainless
steel. In case the connectors are made of brass, the Constructional data
surfaces are usually chrome-plated by means of The products must comply with the standard DIN EN
various galvanic process stages. 1113 and specific Hansgrohe standards.
For the use and application of the product the
respective national provisions at the place of use Name Value Unit
apply, in Germany for example the building codes of Maximum load temperature
42 °C
the federal states and the corresponding national permanent operation
specifications. Maximum load temperature
70 °C
Following standards apply to shower hoses to prove temporary operation
product safety: Flow rate (indications for pressure
> 0,72 m3/h
EN 1113:2015: Sanitary tapware – Shower hoses for range of 1-3 bar)
sanitary tapware for water supply systems of type 1 Sound emissions - dB
and type 2
2.2 Application
Shower hoses are the hoses which connect hand Performance data of the product with respect to its
showers to plumbing fixtures for water supply. They characteristics in accordance with the relevant
are used for showers and bathtubs. technical provision (no CE-marking).
2 Environmental Product Declaration Hansgrohe Group – Shower hoses
2.4 Delivery status
The shower hoses are delivered singularly packaged. 2.7 Environment and health during
The packaging is customized to the size of the product manufacturing
and supplies. Customers can order single products or Hansgrohe SE tries to keep the impact on people and
multiple products with outer packaging. The the environment as low as possible when
dimensions of the products are between manufacturing its products.
25x25x1250 mm and 25x25x2050 mm. Hazards at workplaces are regularly assessed and
reduced to a minimum.
2.5 Base materials/Ancillary materials For example, in basic production, sawing or grinding
work is mainly carried out by robots, and in
The hoses are made of an inner hose and an outer electroplating, chemicals are dosed automatically via
hose. Inner hose made of thermoplastic elastomer appropriate pump stations.
(TPE) - total weight share of approx. 10 %. Outer hose Emissions that are hazardous to health are extracted
made of Polyvinylchloride (PVC) - total weight share of directly at the source and cleaned by filter systems.
approx. 70%. The fittings are made of brass and Workplace and emission limits are regularly monitored
contain between 0.1 % and 1.4 % lead. The material and are far below the prescribed limits.
composition (incl. packaging) of an average shower To reduce environmental impact, water and production
hose is as follows: waste are recycled wherever possible.
In addition, all production sites are certified according
Name Value Unit to the DIN EN ISO standards 14001 (environment),
Brass 14.4 % 50001 (energy), 45001 (occupational health and
Stainless steel 1.9 % safety) and 9001 (quality). Continuous improvement of
Plastic 66.0 % environmental and occupational safety performance is
Cardboard, Paper (packaging) 17.6 % thus guaranteed.
This product contains substances listed in the 2.8 Product processing/Installation
candidate list (date: 17.12.2021) exceeding 0.1 The shower hose is screwed with the union nut and the
percentage by mass: Lead (CAS number 7439-92-1) seal onto the shower fitting or the water connection by
as a component of the brass alloy has been on the hand. And it is also screwed by hand onto the hand
candidate list of the Reach Regulation (Regulation shower with the union nut and the seal (tools: none).
(EC) No. 1907/2006) since 27.06.2018.
2.9 Packaging
This product/article/at least one partial article contains For product protection the shower hoses are
other carcinogenic, mutagenic, reprotoxic (CMR) individually packed in a cardboard box, which consists
substances in categories 1A or 1B which are not on of approximately 80% recycled material. The
the candidate list, exceeding 0.1 percentage by mass: cardboard is always printed with lead-free ink and in
no. some cases additionally coated with a clear topcoat.
The inlay of the packaging consists of folded
Biocide products were added to this construction cardboard, fibre form or plastic bags, depending on the
product or it has been treated with biocide products product.
(this then concerns a treated product as defined by the The packaging can be fully recycled.
(EU) Ordinance on Biocide Products No. 528/2012): All packaged products fit on a reusable euro pallet.
no.
2.6 Manufacture 2.10 Condition of use
To protect the shower hoses and make them durable,
parts of the product are usually chrome-plated.
Nevertheless, there are no unhealthy contaminants in
the water. To ensure the longevity of the product, it
should be used and cleaned regularly.
2.11 Environment and health during use
Our products do not emit any contaminants or
substances that are harmful to the environment or
health during the use phase.
2.12 Reference service life
The quality and durability of our shower hoses are
designed for a product life of about 10 years. Which on
average is approximately the duration of use by the
consumers.
With few exceptions, all products have a five-year
warranty. Furthermore, an after-sale service warranty
No. 1: The TPE inner tube is extruded.
of 15 years is provided.
No. 2: The PVC top layer is applied on the inner tube.
No. 3: The embossing foil chrome is applied on the top
Signs of age of the products can be shown by changed
layer.
surfaces, calcification, or mechanical wearing.
No. 4: The hose is cut in length and assembled with
the connections.
2.13 Extraordinary effects
Any production waste generated is disposed
accordingly.
Fire
3 Environmental Product Declaration Hansgrohe Group – Shower hoses
The products are not classified as building materials 2.14 Re-use phase
(building products) and are not subject to DIN 4102 The shower hoses are not taken back by the
and EN 13501-1. manufacturer for the purpose of reuse. Users can
disassemble the products repeatedly within the
Fire protection reference utilization period and reuse it elsewhere.
Name Value
Building material class - 2.15 Disposal
Burning droplets - The waste code of the product is AVV 20 03 01.
Smoke gas development - Disassembly of the products consists of the same
steps as assembly, in reverse order.
Water All metal components can be recycled (as scrap), all
If a room in which the products offered by Hansgrohe plastic components have a high calorific value and can
are installed is flooded with water, the products are not be incinerated with energy recovery, provided the
affected in their function. components have been separated beforehand. A more
conservative approach is modelled in this EPD
Mechanical destruction considering plastic incineration as the main disposal
If the surface of the coating is destroyed by a route without credits for metal recycling.
mechanical stress, there is a possibility of corrosion.
In the event of mechanical damage, the products may 2.16 Further information
need to be replaced due to possible sharp cut edges. Additional information about our products can be found
at https://www.hansgrohe.com.
3. LCA: Calculation rules
3.1 Declared Unit This module covers the installation process with the
The results of this EPD are valid for the following corresponding packaging waste generated that needs
functional unit: to be disposed of.
Provide sanitary function for one (1) average shower Module B2:
hose unit including packaging, used in accordance with Maintenance expenses are declared in this module
the manufacturer's recommendations for a 10-year life, and consist of weekly cleaning expenses for this
following the manufacturer's operating instructions. An product.
average conditioned shower hose is considered the Module B1, B3-B7:
baseline flow. These modules were considered, but evaluated as not
relevant for the shower hoses and considered as zero.
Weighted averaging based on production tonnages in Modules C1-C4
2020 is chosen as the basis for creating the The modules include the environmental impacts for
environmental profile. 42 different shower hoses were dismantling on the shower hoses and the treatment of
considered. the waste fractions until the end-of-waste status (EoW)
is reached, including the associated transports at the
Functional unit end of the product life cycle.
Name Value Unit Module D
Declared unit 1 pce. Identification of the benefits and costs of the product
Functional unit 1 pce. outside the system boundary. For plastics, these
Functional unit with packaging 0.374 kg consist of energy credits from thermal utilization (C3) in
Packaging 0.071 kg the form of the average European electricity mix or
Weight range of the products 0.206 - thermal energy from natural gas. Recycling of metal
kg
examined 0.546 scrap results in credits of the respective raw materials.
3.3 Estimates and assumptions
Energy and water consumption, material amount for
3.2 System boundary coating as well as waste during production could only
be determined on concrete and existing products and
This average EPD follows the EPD type "cradle to not on the average product. Since the top seller
grave". The following life cycle modules are declared: represents a high proportion of the production volume
Modules A1-A3: and has a similar GWP to the calculated average
The product stage begins with considering the product, the top seller was chosen for the assessment
production of the necessary raw materials and of energy, water, waste and coating. For the
energies, including all corresponding upstream chains incineration with energy recovery (thermal and electric)
and the actual procurement transports. Furthermore, of waste, an r1 value of >0.6 is assumed. The net
the entire manufacturing phase was mapped, including efficiency for the average waste incinerated is between
the treatment of production waste until the end-of- 38 and 44%, depending on the type of waste
waste status (EoW) was reached. Green electricity respectively the disposal data set
from hydropower is used for the manufacturing
processes in Germany. US electricity mix is used for 3.4 Cut-off criteria
the US production site. The effect associated with the neglected mass shares
Module A4: is less than 5 % of the effect categories per module.
All distribution transports (A4) to the customers were The minimum limit of 1 % total mass and the use of
considered. renewable and non-renewable primary energy is not
Module A5: exceeded.
4 Environmental Product Declaration Hansgrohe Group – Shower hoses
3.5 Background data supplies could be assigned to the declared product.
The LCA software GaBi 10.6 was used to model the Energy, water and galvanization process were
life cycle. The entire manufacturing process, as well as assigned to a top-seller representing a large portion of
energy consumption, were modelled on the basis of the product volume. No byproducts are produced and
manufacturerspecific data. no allocation is required.
However, generic background datasets were used for Credits for plastics, paper and cardboard recycled in
the upstream and downstream processes. The majority A5 and metallurgical waste in C3 are credited in
of the background datasets used were taken from the module D.
current version (2021.2) of the GaBi database. Credits for the energy recovery of incinerated
Ecoinvent Version 3.6 (2019) datasets were only used production waste in A1-3, paper, cardboard and
when suitable GaBi datasets were not available. plastics in A5 and plastics and other materials in C3
are credited in module D.
3.6 Data quality Packaging:
The background datasets used for accounting For paper and cardboard, recycling (91 %) and energy
purposes mainly originate from the respective updated recovery (9 %) are considered on a pro rata basis. For
GaBi databases at the time of calculation. plastic, a proportionate recycling (52 %) and energy
The data for the examined products was captured on recovery (48 %) are considered.
the basis of evaluations of internal production and Deconstructed product at the end of life:
environmental data, the collection of LCA relevant 95 % of the non-metallic components are recycled for
data within the supply chain, as well as the evaluation energy recovery and 5 % are disposed of in landfill.
of relevant data for the energy supply. The collected For the metal components, it is assumed that 95 % are
data were checked for plausibility and consistency. sent for incineration with the plastic but without energy
Good representativity can be assumed. recovery and 5 % are disposed of in landfill (C4).
For the assessment of the variability of the results, all
products were balanced in addition to the average 3.9 Comparability
product. Considering modules A1-C4, the variation of Basically, a comparison or an evaluation of EPD data
the GWP indicator value ranges in relation to the is only possible if all the data sets to be compared
declared product between -6 % and +10 %. were created according to EN 15804 and the building
context, respectively the product-specific
3.7 Period under review characteristics of performance, are taken into account.
Life cycle assessment data were collected in 2020.
The background database used is GaBi 10.6 in the
3.8 Allocation database version 2021.2
For the production process of the different product
groups nearly all raw materials, precursors and
4. LCA: Scenarios and additional technical information
Characteristic product properties Name Value Unit
Information on biogenic carbon Packaging waste Paper,
0.071 kg
cardboard and plastic
Information on describing the biogenic Carbon Use or application of the installed product (B1) see
Content at factory gate section 2.12 "Use"
Name Value Unit
Biogenic Carbon Content in No emissions are expected.
- kg C
product -
Biogenic Carbon Content in Maintenance (B2)
0.0245 kg C
accompanying packaging For module B2, it is assumed that a weekly cleaning of
the product takes place, with 0.5 litre of water
containing 1.5 % soap.
Name Value Unit
Water consumption/Cycle weekly 0.5 Liter/cycle
Transport to the building site (A4) Soap concentration 1.5 %
Name Value Unit Number/R
Maintenance cycle 520
Transport distance (Truck) 613 km SL
Capacity utilisation, including empty Water consumption 0.26 m3
55 %
runs (Truck) Auxiliary Soap (Tensides) 3.9 kg
Transport distance (Container Ship) 1847 km
Capacity utilisation (Container Ship) 80 %
Hansgrohe SE declares a Service Life of 10
Installation into the building (A5) years as an empirical value for the shower hoses when
The shower hose with union nut and seal is first used in accordance with the care instructions. This
screwed onto the shower fitting or water connection by value is based on their technical service centre's
hand. Then the hose is screwed onto the hand shower statistics on service life in the market and complaints.
by hand using the union nut and seal. No additional
resources or energy are required for this. The Service life
packaging is disposed either by recycling or Name Value Unit
incineration. Life Span according to the
10 a
manufacturer
5 Environmental Product Declaration Hansgrohe Group – Shower hoses
End of life (C1-C4)
Name Value Unit
Collected as mixed construction waste 0.303 kg
Energy recovery (Plastics, Metal) 0.288 kg
Landfilling (Plastics, Metal) 0.015 kg
Reuse, recovery and/or recycling potentials (D),
relevant scenario information
In module D, the credits from the energetic energy
recovery of the packaging materials (resulting from
module A5) and of the plastic incineration at end of life
are shown.
6 Environmental Product Declaration Hansgrohe Group – Shower hoses
5. LCA: Results
The following table shows the result of the LCA for 1 piece of an average shower hose. The results in the B-
module are based on a lifetime of 10 years.
DESCRIPTION OF THE SYSTEM BOUNDARY (X = INCLUDED IN LCA; ND = MODULE OR INDICATOR NOT
DECLARED; MNR = MODULE NOT RELEVANT)
BENEFITS AND
CONSTRUCTI LOADS
PRODUCT STAGE ON PROCESS USE STAGE END OF LIFE STAGE BEYOND THE
STAGE SYSTEM
BOUNDARIES
7 Environmental Product Declaration Hansgrohe Group – Shower hoses
lairetam
waR
ylppus tropsnarT
gnirutcafunaM
eht
morf
tropsnarT
etis
eht
ot
etag
ylbmessA esU
ecnanetniaM
riapeR
tnemecalpeR tnemhsibrufeR
ygrene
lanoitarepO esu
retaw
lanoitarepO esu
noitcurtsnoc-eD
noitilomed tropsnarT
gnissecorp
etsaW
lasopsiD -esueR -yrevoceR -gnilcyceR laitnetop
A1 A2 A3 A4 A5 B1 B2 B3 B4 B5 B6 B7 C1 C2 C3 C4 D
X X X X X X X MNR MNR MNR X X X X X X X
RESULTS OF THE LCA - ENVIRONMENTAL IMPACT according to EN 15804+A2: 1 piece average shower
hose incl. packaging
Core Indicator Unit A1-A3 A4 A5 B1 B2 B6 B7 C1 C2 C3 C4 D
GWP-total [kg CO2-Eq.] 5.94E-1 2.55E-2 1.01E-1 0.00E+0 1.28E+1 0.00E+0 0.00E+0 0.00E+0 5.15E-3 6.15E-1 1.02E-3 -3.11E-1
GWP-fossil [kg CO2-Eq.] 6.83E-1 2.53E-2 1.11E-2 0.00E+0 9.80E+0 0.00E+0 0.00E+0 0.00E+0 5.11E-3 6.15E-1 1.02E-3 -2.21E-1
GWP-biogenic [kg CO2-Eq.] -8.99E-2 0.00E+0 8.99E-2 0.00E+0 0.00E+0 0.00E+0 0.00E+0 0.00E+0 0.00E+0 0.00E+0 0.00E+0 -8.99E-2
GWP-luluc [kg CO2-Eq.] 9.40E-4 1.60E-4 1.38E-5 0.00E+0 3.01E+0 0.00E+0 0.00E+0 0.00E+0 4.19E-5 1.26E-4 8.74E-7 -3.26E-4
ODP [kg CFC11-Eq.] 5.73E-10 4.45E-18 5.46E-17 0.00E+0 5.43E-7 0.00E+0 0.00E+0 0.00E+0 1.01E-18 1.59E-12 2.44E-18 -1.39E-9
AP [mol H+-Eq.] 1.84E-3 2.46E-4 8.16E-6 0.00E+0 3.32E-2 0.00E+0 0.00E+0 0.00E+0 8.57E-6 1.55E-4 3.07E-6 -3.13E-4
EP-freshwater [kg P-Eq.] 1.14E-5 5.93E-8 1.83E-8 0.00E+0 2.90E-4 0.00E+0 0.00E+0 0.00E+0 1.52E-8 1.45E-7 1.60E-7 -3.59E-6
EP-marine [kg N-Eq.] 4.60E-4 6.92E-5 2.72E-6 0.00E+0 7.57E-3 0.00E+0 0.00E+0 0.00E+0 3.37E-6 5.07E-5 7.07E-7 -1.07E-4
EP-terrestrial [mol N-Eq.] 4.88E-3 7.64E-4 3.27E-5 0.00E+0 9.04E-2 0.00E+0 0.00E+0 0.00E+0 3.86E-5 6.42E-4 7.75E-6 -1.13E-3
POCP [kg NMVOC-Eq.] 1.79E-3 1.87E-4 6.86E-6 0.00E+0 3.02E-2 0.00E+0 0.00E+0 0.00E+0 7.65E-6 1.46E-4 2.25E-6 -2.87E-4
ADPE [kg Sb-Eq.] 2.74E-5 1.90E-9 7.83E-10 0.00E+0 1.05E-5 0.00E+0 0.00E+0 0.00E+0 4.54E-10 1.36E-8 6.99E-11 -5.28E-7
ADPF [MJ] 1.63E+1 3.30E-1 4.83E-2 0.00E+0 2.26E+2 0.00E+0 0.00E+0 0.00E+0 6.83E-2 1.01E+0 1.48E-2 -3.39E+0
[m³ world-Eq
WDP 9.81E-2 1.90E-4 1.89E-3 0.00E+0 3.47E+0 0.00E+0 0.00E+0 0.00E+0 4.76E-5 4.89E-2 -1.24E-5 -4.07E-2
deprived]
GWP = Global warming potential; ODP = Depletion potential of the stratospheric ozone layer; AP = Acidification potential of land and water; EP =
Caption Eutrophication potential; POCP = Formation potential of tropospheric ozone photochemical oxidants; ADPE = Abiotic depletion potential for non-
fossil resources; ADPF = Abiotic depletion potential for fossil resources; WDP = Water (user) deprivation potential
RESULTS OF THE LCA - INDICATORS TO DESCRIBE RESOURCE USE according to EN 15804+A2: 1 piece
average shower hose incl. packaging
Indicator Unit A1-A3 A4 A5 B1 B2 B6 B7 C1 C2 C3 C4 D
PERE [MJ] 1.21E+0 1.52E-2 1.14E+0 0.00E+0 4.68E+1 0.00E+0 0.00E+0 0.00E+0 3.93E-3 2.51E-1 1.07E-3 -1.73E+0
PERM [MJ] 1.13E+0 0.00E+0 -1.13E+0 0.00E+0 0.00E+0 0.00E+0 0.00E+0 0.00E+0 0.00E+0 0.00E+0 0.00E+0 0.00E+0
PERT [MJ] 2.34E+0 1.52E-2 1.56E-2 0.00E+0 4.68E+1 0.00E+0 0.00E+0 0.00E+0 3.93E-3 2.51E-1 1.07E-3 -1.73E+0
PENRE [MJ] 9.61E+0 3.31E-1 2.65E-1 0.00E+0 2.26E+2 0.00E+0 0.00E+0 0.00E+0 6.85E-2 7.16E+0 3.38E-1 -3.39E+0
PENRM [MJ] 6.69E+0 0.00E+0 -2.16E-1 0.00E+0 0.00E+0 0.00E+0 0.00E+0 0.00E+0 0.00E+0 -6.15E+0 -3.23E-1 0.00E+0
PENRT [MJ] 1.63E+1 3.31E-1 4.83E-2 0.00E+0 2.26E+2 0.00E+0 0.00E+0 0.00E+0 6.85E-2 1.01E+0 1.48E-2 -3.39E+0
SM [kg] 9.90E-2 0.00E+0 0.00E+0 0.00E+0 0.00E+0 0.00E+0 0.00E+0 0.00E+0 0.00E+0 0.00E+0 0.00E+0 2.76E-2
RSF [MJ] 0.00E+0 0.00E+0 0.00E+0 0.00E+0 0.00E+0 0.00E+0 0.00E+0 0.00E+0 0.00E+0 0.00E+0 0.00E+0 0.00E+0
NRSF [MJ] 0.00E+0 0.00E+0 0.00E+0 0.00E+0 0.00E+0 0.00E+0 0.00E+0 0.00E+0 0.00E+0 0.00E+0 0.00E+0 0.00E+0
FW [m³] 5.59E-3 1.75E-5 5.13E-5 0.00E+0 8.10E-2 0.00E+0 0.00E+0 0.00E+0 4.50E-6 1.27E-3 1.40E-7 -1.35E-3
PERE = Use of renewable primary energy excluding renewable primary energy resources used as raw materials; PERM = Use of
renewable primary energy resources used as raw materials; PERT = Total use of renewable primary energy resources; PENRE = Use of
non-renewable primary energy excluding non-renewable primary energy resources used as raw materials; PENRM = Use of non-
Caption
renewable primary energy resources used as raw materials; PENRT = Total use of non-renewable primary energy resources; SM = Use
of secondary material; RSF = Use of renewable secondary fuels; NRSF = Use of non-renewable secondary fuels; FW = Use of net fresh
water
RESULTS OF THE LCA – WASTE CATEGORIES AND OUTPUT FLOWS according to EN 15804+A2:
1 piece average shower hose incl. packaging
Indicator Unit A1-A3 A4 A5 B1 B2 B6 B7 C1 C2 C3 C4 D
HWD [kg] 3.68E-7 1.43E-11 1.01E-11 0.00E+0 4.25E-3 0.00E+0 0.00E+0 0.00E+0 3.61E-12 1.91E-10 2.66E-12 -1.00E-9
NHWD [kg] 2.06E-2 4.80E-5 5.87E-4 0.00E+0 3.29E-1 0.00E+0 0.00E+0 0.00E+0 1.08E-5 1.28E-2 1.51E-2 -1.68E-3
RWD [kg] 2.69E-4 5.51E-7 2.82E-6 0.00E+0 2.06E-3 0.00E+0 0.00E+0 0.00E+0 1.24E-7 3.31E-5 1.71E-7 -1.21E-4
CRU [kg] 0.00E+0 0.00E+0 0.00E+0 0.00E+0 0.00E+0 0.00E+0 0.00E+0 0.00E+0 0.00E+0 0.00E+0 0.00E+0 0.00E+0
MFR [kg] 0.00E+0 0.00E+0 6.23E-2 0.00E+0 0.00E+0 0.00E+0 0.00E+0 0.00E+0 0.00E+0 0.00E+0 0.00E+0 0.00E+0
MER [kg] 0.00E+0 0.00E+0 0.00E+0 0.00E+0 0.00E+0 0.00E+0 0.00E+0 0.00E+0 0.00E+0 0.00E+0 0.00E+0 0.00E+0
EEE [MJ] 2.73E-4 0.00E+0 2.88E-2 0.00E+0 0.00E+0 0.00E+0 0.00E+0 0.00E+0 0.00E+0 7.32E-1 7.06E-8 0.00E+0
EET [MJ] 5.57E-4 0.00E+0 5.17E-2 0.00E+0 0.00E+0 0.00E+0 0.00E+0 0.00E+0 0.00E+0 1.33E+0 0.00E+0 0.00E+0
HWD = Hazardous waste disposed; NHWD = Non-hazardous waste disposed; RWD = Radioactive waste disposed; CRU = Components
Caption for re-use; MFR = Materials for recycling; MER = Materials for energy recovery; EEE = Exported electrical energy; EET = Exported
thermal energy
RESULTS OF THE LCA – additional impact categories according to EN 15804+A2-optional:
1 piece average shower hose incl. packaging
Indicator Unit A1-A3 A4 A5 B1 B2 B6 B7 C1 C2 C3 C4 D
[Disease
PM 1.76E-8 3.85E-9 5.52E-11 0.00E+0 1.65E-6 0.00E+0 0.00E+0 0.00E+0 5.35E-11 3.58E-9 3.06E-11 -4.18E-9
Incidence]
[kBq U235-
IRP 5.00E-2 8.04E-5 3.77E-4 0.00E+0 1.07E+0 0.00E+0 0.00E+0 0.00E+0 1.82E-5 3.42E-3 2.46E-5 -1.25E-2
Eq.]
ETP-fw [CTUe] 1.04E+1 2.44E-1 2.42E-2 0.00E+0 1.00E+2 0.00E+0 0.00E+0 0.00E+0 5.07E-2 7.93E-1 1.26E-2 -1.03E+0
HTP-c [CTUh] 1.13E-8 4.85E-12 7.57E-13 0.00E+0 1.10E-8 0.00E+0 0.00E+0 0.00E+0 1.03E-12 3.22E-11 6.12E-13 -5.45E-11
HTP-nc [CTUh] 3.02E-8 2.52E-10 3.53E-11 0.00E+0 3.74E-7 0.00E+0 0.00E+0 0.00E+0 5.45E-11 3.30E-9 5.25E-11 -2.01E-9
SQP [-] 3.39E+0 8.95E-2 1.70E-2 0.00E+0 1.59E+2 0.00E+0 0.00E+0 0.00E+0 2.35E-2 2.40E-1 1.02E-3 -5.64E+0
PM = Potential incidence of disease due to PM emissions; IR = Potential Human exposure efficiency relative to U235; ETP-fw = Potential
Caption comparative Toxic Unit for ecosystems; HTP-c = Potential comparative Toxic Unit for humans (cancerogenic); HTP-nc = Potential
comparative Toxic Unit for humans (not cancerogenic); SQP = Potential soil quality index
6. LCA: Interpretation
The environmental burdens from the transports
The dominance analysis shows that module B2 in (modules A4 and C2) account for less than 1 % of the
particular is the dominant life cycle stage, due to the total burdens of the respective indicators in all cases.
demand of soap and water for cleaning. The module The possible potentials of avoided loads of subsequent
A1-A3 has the second most input regarding GWP systems (module D) lie outside the considered system
total
(0.59 kg CO -eq.). This is mainly caused by the boundaries and relate exclusively to credits from
2
provision of plastic (PVC) for the production of the recycling and thermal recycling by means of
shower hose at the production site (0.43 kg CO -eq.) incineration with energy recovery of the different
2
ADPE differs from the other indicators. The provision materials.
of brass in A1-A3 has the largest contribution. For the assessment of the variability of the results, all
The end-of-life stage (module C1-C4) only has a other products were balanced in addition to the
noteworthy influence on the indicators GWP and average product. Considering modules A1-C4, the
total
WDP. Here, these indicators are each influenced variation of the GWP indicator value ranges in
fossil
primarily by the thermal treatment of plastics. The end- relation to the declared product between -6 % and +10
of-life stage has no significant influence on the other %.
environmental indicators.
7. Requisite evidence
The drinking water regulation determines the quality of All materials used by Hansgrohe SE, which are in
drinking water at the point of withdrawal. This result in contact with drinking water, fulfill the drinking water
requirements for used materials in drinking water regulation.
installations in general and therefore in sanitary fittings Regulations for metals (Europe-wide):
in particular.
8 Environmental Product Declaration Hansgrohe Group – Shower hoses
 Acceptance of metallic materials used for  Ceramics: draft assessment basis for
products in contact with drinking water: 4MS enamels and ceramic materials: assessment
Common Approach basis for enamels and ceramic materials in
contact with drinking water (enamel/ceramic
- Part A – Procedure for the acceptance assessment basis)
- Part B – 4MS Common Composition List  Lubricants: Guideline for the hygienic
assessment of lubricants in contact with
 Metal recommendation of the federal drinking water (sanitary lubricants), (Lubricant
environment agency: metal materials suitable Guideline)
for drinking water hygiene
Regulation for other materials (France):
Regulations for other materials (Germany):  ACS: Attestation de Conformité Sanitaire
 KTW: Assessment basis for plastics and other (plastics, elastomers, metals)
organic materials in contact with drinking
water
Regulation for other materials (UK):
 Elastomer guideline: Guideline for the
 BS 69 20: Suitability of non-metallic products
hygienic assessment of elastomers in contact
for use in contact with water intended for
with drinking water
human consumption with regard to their effect
 Thermoplastic elastomers: Recommendation on the quality of water (plastics, elastomers)
for the hygienic assessment of products made
of thermoplastic elastomers in contact with
Products of the Hansgrohe SE are therefore uncritical
drinking water (TPE transition
to use with any drinking water.
recommendation)
8. References
Standards
DIN EN ISO 45001
DIN EN 1113 DIN EN ISO 45001:2018: Occupational health and
DIN EN 1113:2015-06, Sanitary tapware - Shower safety management systems — Requirements with
hoses for sanitary tapware for water supply systems of guidance for use. 2018-03
type 1 and type 2 - General technical specification;
German version EN 1113:2015 DIN EN ISO 50001
DIN EN ISO 50001:2018: Energy management
DIN 4102-1 systems — Requirements with guidance for use. 2018-
DIN 4102-1: Fire behaviour of building materials and 08
building components - Part 1: Building materials;
concepts, requirements and tests. 1998-05 Further References
DIN EN ISO 9004 AVV
DIN EN ISO 9004:2018: Quality management — Draft General administrative provision relating to the
Quality of an organization — Guidance to achieve Order on the European list of wastes (Waste List Order
sustained success. 2018-04 – German designation: AVV) of 10 December 2001.
DIN EN 13501-1 ECHA
DIN EN 13501-1:2019-05: Fire classification of European Chemicals Agency (ECHA) Candidate List of
construction products and building elements - Part 1: Substances of Very High Concern (SVHC) for
Classification using data from reaction to fire tests; Authorisation https://echa.europa.eu/de/candidate-list-
German version EN 13501-1:2018 table
DIN EN ISO 14001 Ecoinvent
DIN EN ISO 14001:2015, Environmental management Ecoinvent 3.6. Database for Life Cycle Assessment.
systems — Requirements with guidance for use, 2015- Wernet, G., Bauer, C., Steubing, B., Reinhard, J.,
09 Moreno-Ruiz, E., and Weidema, B., 2016. The
ecoinvent database version 3 (part I): overview and
DIN EN ISO 14025 methodology. The International Journal of Life Cycle
DIN EN ISO 14025: Environmental labels and Assessment, [online] 21(9), pp.
declarations - Type III environmental declarations -
Principles and procedures, 2011-10 EU Ordinance on biocide Products No. 528/2012
European Parliament, 2012. Regulation (EU) no
DIN EN 15804 528/2012 of the European parliament and of the
DIN EN 15804:2012+A2:2019+AC:2021: Sustainability council of 22 May 2012 concerning the making
of construction works - Environmental product available on the market and use of biocidal products
declarations - Core rules for the product category of
construction products; German version EN GaBi
15804:2012+A2:2019+AC:2021
9 Environmental Product Declaration Hansgrohe Group – Shower hoses
GaBi 10.6, GaBi Software System and Database for assessment and requirements on the project report.
Life Cycle Engineering, Sphera Solutions GmbH, Version 2.1 (11.2021)
1992-2021
PCR Part B
IBU 2021 Institut Bauen und Umwelt e.V. (IBU). Requirements
General Instructions for the EPD programme of Institut on the EPD for Bathroom fittings and showers,
Bauen und Umwelt e.V. Version 2.0, 03/2022
Berlin: Institut Bauen und Umwelt e.V.,
2021
www.ibu-epd.com
PCR Part A
Institut Bauen und Umwelt e.V. (IBU), 2021. Product
Category Rules for Building-Related Products and
Services. Part A: Calculation rules for the life cycle
10 Environmental Product Declaration Hansgrohe Group – Shower hoses
Publisher
Institut Bauen und Umwelt e.V. Tel +49 (0)30 3087748- 0
Hegelplatz 1 Fax +49 (0)30 3087748- 29
10117 Berlin Mail info@ibu-epd.com
Germany Web www.ibu-epd.com
Programme holder
Institut Bauen und Umwelt e.V. Tel +49 (0)30 - 3087748- 0
Hegelplatz 1 Fax +49 (0)30 – 3087748 - 29
10117 Berlin Mail info@ibu-epd.com
Germany Web www.ibu-epd.com
Author of the Life Cycle
Assessment Tel +49 421 70 90 84 33
brands & values GmbH Fax +49 421 70 90 84 35
Altenwall 14 Mail info@brandsandvalues.com
28195 Bremen Web www.brandsandvalues.com
Germany
Owner of the Declaration
Hansgrohe Group Tel +49 7836 51-0
Auestr. 5-9 Fax +49 7836 51-1300
77761 Schiltach Mail info@hansgrohe-group.com
Germany Web http://www.hansgrohe-
group.com
