ENVIRONMENTAL PRODUCT DECLARATION
as per ISO 14025 and EN 15804+A2
Owner of the Declaration Hansgrohe Group
Programme holder Institut Bauen und Umwelt e.V. (IBU)
Publisher Institut Bauen und Umwelt e.V. (IBU)
Declaration number EPD-HAN-20230022-ICC1-EN
Issue date 24.02.2023
Valid to 23.02.2028
Showerpipes
Hansgrohe Group
www.ibu-epd.com | https://epd-online.com
Umwelt Produktdeklaration Name des Herstellers – Name des Produkts
1. General Information
Hansgrohe Group Showerpipes
Programme holder Owner of the declaration
IBU – Institut Bauen und Umwelt e.V. Hansgrohe Group
Hegelplatz 1 Auestraße 5 - 9
10117 Berlin 77761 Schiltach
Germany Germany
Declaration number Declared product / declared unit
EPD-HAN-20230022-ICC1-EN One (1) piece of an average showerpipe incl.
packaging
This declaration is based on the product Scope:
category rules: This average EPD was determined on the basis of a
Fittings and showers, 07.2014 weighted average of production volume from 2021 and
(PCR checked and approved by the SVR) relates to the plants in Offenburg, Willstätt and
Schiltach, Germany, Shanghai, China and Alpharetta,
USA. This average EPD is valid for the whole product
Issue date
group of chrome plated showerpipes. The EPD was
24.02.2023
formed from >96% of the products involved in the sales
quantity.
Valid to
23.02.2028
The owner of the declaration shall be liable for the
underlying information and evidence; the IBU shall not
be liable with respect to manufacturer information, life
cycle assessment data and evidences.
The EPD was created according to the specifications
of EN 15804+A2. In the following, the standard will be
simplified as EN 15804.
Verification
The standard EN 15804 serves as the core PCR
Independent verification of the declaration and data
according to ISO 14025:2011
Dipl. Ing. Hans Peters internally x externally
(chairman of Institut Bauen und Umwelt e.V.)
Dr. Alexander Röder Dr Naeem Adibi
(Managing Director Institut Bauen und Umwelt e.V.)) (Independent verifier)
2. Product
2.1 Product description/Product definition Following standards depending on the operating
A showerpipe is a combination of a shower valve, mechanism may apply to showerpipes to prove
shower hose and/or pipe connection and head shower product safety:
and/or hand shower.
 EN 816:2017: Sanitary tapware – Automatic
Showerpipes essentially comprise of a metal housing shut-off valves PN 10
in most cases made of brass, a plastic valve with
 EN 817:2008: Sanitary tapware – Mechanical
ceramic discs or thermostatic cartridge, and several
mixing valves (PN 10)
assembly parts of various materials. The pipe surface
is usually chrome-plated by means of various galvanic  EN 200:2008: Sanitary tapware – Single taps
process stages. Roughs mainly comprise of brass and combination taps for water supply
materials. systems of type 1 and type 2
 EN 1111:2018: Sanitary tapware –
For the use and application of the product the
Thermostatic mixing valves (PN 10)
respective national provisions at the place of use
 EN 1112:2008: Sanitary tapware – Shower
apply, in Germany for example the building codes of
the federal states and the corresponding national outlets for sanitary tapware for water supply
specifications. systems of type 1 and type 2
 EN 1113:2015: Sanitary tapware – Shower
The products comply with the applicable standards and
hoses for sanitary tapware for water supply
regulations listed below.
systems of type 1 and type 2
2 Environmental Product Declaration Hansgrohe Group – Showerpipes
 ISO 3822: Acoustics – Laboratory tests on This product/article/at least one partial article contains
noise emission from appliances and other CMR substances in categories 1A or 1B which
are not on the candidate list, exceeding 0.1 percentage
equipment used in water supply installations
by mass: no.
2.2 Application Biocide products were added to this construction
Showerpipes are a combination of a faucet or product or it has been treated with biocide products
thermostat, a overhead shower and a hand shower. (this then concerns a treated product as defined by the
Combined with hoses and riser pipe and pipe bend. (EU) Ordinance on Biocide Products No.
They are used in bathrooms for showering or in 528/2012): no.
bathtubs.
2.6 Manufacture
2.3 Technical Data Faucet or thermostat:
Constructional data
Name Value Unit
Maximum load temperature permanent
65 °C
operation
Maximum load temperature temporary
90 °C
operation
Dependi
ng on
Flow rate (indications for pressure the
m3/h
range of 1-3 bar) product
0,09 to
1,2
Sound emissions - dB
Performance data of the product with respect to its
characteristics in accordance with the relevant No. 1: The sand core for the base body is made.
technical provision (no CE-marking). No. 2: The body of the faucet is cast from brass using
the sand core.
2.4 Delivery status No. 3: After casting, the brass body is grinded and
The showerpipes are delivered singularly packaged. polished.
The packaging is customized to the size of the product No. 4: To protect the product and make it durable, the
and supplies. Customers can order single products or body is galvanized with chrome.
multiple products with outer packaging. The products No. 5: Meanwhile, the individual parts of the cartridge
with the smallest and the largest volume have are assembled.
dimensions between 145x31x1135 mm and No. 6: The product parts (chrome plated brass body,
385x280x1165 mm. cartridge, chrome plated handle and others) are
lasered and assembled.
2.5 Base materials/Ancillary materials No. 7: The preassembled product is packed together
with the remaining components (like s-connectors and
The material composition (incl. packaging) of an escutcheon).
average showerpipe is as follows:
Overhead shower:
Name Value Unit
Brass 42.4 %
Cardboard, Paper 26.8 %
Plastic 14.4 %
Zinc 5.2 %
Stainless steel 4.5 %
Acrylonitrile butadiene styrene 4.0 %
Other metals 1.7 %
Other material 0.6 %
Aluminium 0.4 %
Steel 0.1 %
No. 1: The plastic jet body is injected.
The parts which are made of brass contain between
No. 2: The plastic upper part of housing is injected.
0.2 and 1.4% lead.
No. 3: The upper part of housing is galvanized.
This product contains substances listed in the
No. 4: The plastic thread nipple is injected.
candidate list (date: 17.12.2021) exceeding 0.1
No. 5: All the parts are assembled and packed.
percentage by mass: Lead (CAS number 7439-92-1)
as a component of the brass alloy has been on the
Hand shower:
candidate list of the Reach Regulation (Regulation
(EC) No. 1907/2006) since 27.06.2018.
3 Environmental Product Declaration Hansgrohe Group – Showerpipes
Hazards at workplaces are regularly assessed and
reduced to a minimum.
For example, in basic production, sawing or grinding
work is mainly carried out by robots, and in
electroplating, chemicals are dosed automatically via
appropriate pump stations.
Emissions that are hazardous to health are extracted
directly at the source and cleaned by filter systems.
Workplace and emission limits are regularly monitored
and are far below the prescribed limits.
To reduce environmental impact, water and production
waste are recycled wherever possible.
In addition, all production sites are certified according
to the DIN EN
ISO standards 14001 (environment), 50001 (energy), 4
5001 (occupational health and safety)
and 9001 (quality). Continuous improvement of
environmental and occupational safety performance is
thus guaranteed.
2.8 Product processing/Installation
Remove building protection caps.
No. 1: The plastic handle of the hand showers is
Seal the transitions from the connections to the tiles
injected.
(tools: water + dishwashing liquid).
No. 2: The handle is galvanized with chrome.
Adjust the s-connectors to installation length (tool:
No. 3: The plastic inlet housing is injected.
handsaw).
No. 4: The plastic pipe bow is injected.
Screw in and seal the s-connectors and align them
No. 5: The plastic distributor is injected.
(tool: wrench, spirit level).
No. 6: Meanwhile, the plastic jet body is injected.
Screw the escutcheon over the s-connectors. And
No. 7: The distributor and the jet body are
screw on the fitting (tool: wrench).
preassembled.
Make holes in the pipe for the wall bracket (tool: drilling
No. 8: All the parts are assembled and packed.
machine).
Seal the holes with silicone (tool: silicon injector).
Hose:
Attach the pipe to the bracket and screw on the shower
head (tool: hexagonal offset screwdriver, wrench).
Screw the shower hose with union nut and seal onto
the shower fitting or water connection by hand.
Screw the shower hose with union nut and seal onto
the hand shower by hand.
In the end the water temperature is adjusted by setting
the cartridge (tools: standard hexagonal offset
screwdriver).
2.9 Packaging
For product protection the showerpipes are individually
packed in a cardboard box, which consists of
approximately 80% recycled material. The cardboard is
always printed with lead-free ink and in some cases
additionally coated with clear topcoat. The inlay of the
No. 1: The PVC inner tube is extruded. packaging consists of folded cardboard, fiber form or
No. 2: The PVC top layer is applied on the inner tube. plastic bags, depending on the product.
No. 3: The embossing foil chrome is applied on the top The packaging can be fully recycled.
layer.
No. 4: The hose is cut in length and assembled with
the connections. 2.10 Condition of use
To protect the showerpipes and make them durable,
Packaging: the product is usually chrome-plated. Nevertheless,
In the end all components are packed together with there are no unhealthy contaminants in the water. To
some additional parts like riser pipe and pipe bend. ensure the longevity of the product, it should be used
and cleaned regularly.
Any production waste generated is disposed
accordingly. In individual cases, the production may 2.11 Environment and health during use
differ slightly from the procedure (for example, if the Our products do not emission any contaminants or
handle is not chrome-plated). substances that are harmful to the environment or
health during the use phase.
2.7 Environment and health during
manufacturing 2.12 Reference service life
Hansgrohe SE tries to keep the impact on people and The quality and durability of our showerpipes is
the environment as low as possible when designed for a product life of about 20 years. Which on
manufacturing its products.
4 Environmental Product Declaration Hansgrohe Group – Showerpipes
average is approximately the duration of use by the
consumers. Mechanical destruction
Nevertheless, it is possible that some parts are needed If the surface of the coating is destroyed by a
to be changed earlier (like shower hoses). mechanical stress, there is a possibility of corrosion.
With few exceptions, all products have a five-year In the event of mechanical damage, the products may
warranty. Furthermore, an after-sale service warranty need to be replaced due to possible sharp cut edges.
of 15 years is provided.
2.14 Re-use phase
The showerpipes are not taken back by the
2.13 Extraordinary effects manufacturer for the purpose of reuse. Users can
disassemble the products repeatedly within the
Fire reference utilization period and reuse it elsewhere.
The products are not classified as building materials
(building products) and are not subject to DIN 4102 2.15 Disposal
and EN 13501-1. The waste code of the product
is AVV 20 03 01. Disassembly of the products consists
Fire protection of the same steps as assembly, in reverse order.
Name Value All metal components can be recycled (as scrap).
Building material class - All plastic components have a high calorific value and
Burning droplets - can be sent for thermal recycling.
Smoke gas development - In countries where no thermal recycling or substance
recycling is established, disposal takes place via the
Water waste incineration plant.
If a room in which the products offered by Hansgrohe
are installed is flooded with water, the products are not 2.16 Further information
affected in their function. Additional information about our products can be found
There will be no environmental impact. at https://www.hansgrohe.com.
3. LCA: Calculation rules
3.1 Declared Unit for the Chinese production site, although electricity
The results of this EPD are valid for the following from photovoltaic is partly used there.
functional unit: Module A4:
Provide sanitary function for one (1) average All distribution transports to the customers were
showerpipe unit used in accordance with the considered.
manufacturer's recommendations for a 20-year life, Module A5:
following the manufacturer's operating instructions. An This module covers the installation process with the
average conditioned showerpipe is considered the corresponding packaging waste generated that needs
baseline flow. to be disposed.
Modules B1 & B3-B5:
Weighted averaging based on production tonnages in These modules were considered, but evaluated as not
2021 is chosen as basis for creating the environmental relevant for the products and considered as zero.
profile. 150 different showerpipes were considered. Module B2:
Maintenance expenses are declared in this module
Functional unit and consist of weekly cleaning expenses for this
Name Value Unit product.
Declared unit 1 pce. Module B6:
Functional unit 1 pce. This module considers the energy input required to
Functional unit with packaging 6.73 kg bring water to a certain temperature for the use of a
Packaging 1.86 kg gas low temperature boiler (scenario B6/1) and for the
Weight range of the products 4.48 - use of an electric instantaneous water heater (scenario
kg
examined 16.18 B6/2).
Module B7:
This module considers the water consumption that can
be expected depending on the function of the product
3.2 System boundary family.
This representative EPD follows the EPD type "cradle Modules C1-C4:
to gate - with options". The following life cycle modules The modules include the environmental impacts for
are declared: dismantling of the products and the treatment of the
Modules A1-A3: waste fractions until the end-of-waste status (EoW) is
The product stage begins with considering the reached, including the associated transports at the end
production of the necessary raw materials and of the product life cycle.
energies, including all corresponding upstream chains Module D:
and the actual procurement transports. Furthermore, Identification of the benefits and costs of the product
the entire manufacturing phase was mapped, including outside the system boundary. For waste, paper and
the treatment of production waste until the end-of- plastics, these consist of energy credits from thermal
waste status (EoW) was reached. Green electricity utilization (A3, A5 and C3) in the form of the average
from hydropower is used for the manufacturing European electricity mix or thermal energy from natural
processes in Germany. US electricity mix is used for gas. Recycling of paper, plastic and metal scrap
the US production site. Chinese electricity mix is used results in credits of the respective raw materials for the
5 Environmental Product Declaration Hansgrohe Group – Showerpipes
primary material portion of the input. The loads of the product. See at chapter 6 for explanation of the
waste incineration and recycling processes are variability.
assigned to the respective modules (A3, A5 and C3)
and not to module D. 3.7 Period under review
Life cycle assessment data were collected in 2021.
3.3 Estimates and assumptions
Energy and water consumption, material amount for 3.8 Allocation
coating as well as waste during production could only For the production process nearly all raw materials,
be determined on concrete, existing products and not precursors and supplies could be assigned to the
on the average product. The highest value of all inputs declared product. Energy, water, galvanization process
and outputs for energy, waste and coating of the top and production waste were assigned to the highest
seller, the lightest and the heaviest product was used value of either the heaviest, lightest or most sold
for the calculation of energy, water, waste and coating. product of the product group. No byproducts are
For the incineration with energy recovery (thermal and produced and no allocation is required.
electric) of waste, an r1 value of > 0.6 is assumed. The Some of the brass losses from brass processing in
net efficiency for the average waste incinerated is module A3 are directly reused by Hansgrohe and are
between 38 % and 44 %, depending on the type of modelled as a closed loop. Another part of the brass
waste respectively the disposal data set. losses (brass particles and dusts) is disposed of as
waste (without debits and credits).
3.4 Cut-off criteria Credits for plastics, paper and cardboard recycled in
The effect associated with the neglected mass shares A5 and metallurgical waste in C3 are credited in
is less than 5% of the effect categories per module. module D.
The minimum limit of 1% total mass and the use of Credits for the energy recovery of incinerated
renewable and nonrenewable primary energy is not production waste in A1-3, paper, cardboard and
exceeded. plastics in A5 and plastics and other materials in C3
are credited in module D.
3.5 Background data The loads for waste water treatment and waste
The LCA software GaBi 10.6 was used to model the disposal of core sand, waste oil and hazardous waste
life cycle. The entire manufacturing process, as well as from the manufacturing phase are allocated to module
energy consumption, were modelled on the basis of A3.
manufacturer specific data. Packaging:
However, generic background datasets were used for For paper and cardboard, recycling (91 %) and energy
the upstream and downstream processes. The majority recovery (9 %) are considered on a pro rata basis. For
of the background datasets used were taken from the plastic, a proportionate recycling (52 %), energy
current version (2021.2) of recovery (48 %) considered, based on Eurostat.
the GaBi database. Ecoinvent Version 3.6 (2019) Deconstructed product at the end of life:
datasets were only used when suitable GaBi datasets Since the product is predominantly made of metal, it is
were not available. assumed that most of its metallic components are
recycled. 95 % of the non-metallic components are
3.6 Data quality incinerated with energy recovery and 5 % are disposed
The background datasets used for accounting in landfill. For the metal components, it is assumed that
purposes mainly originate from the respective updated 90 % are sent for material recycling, 5 % for
GaBi databases at the time of calculation. The data for incineration with energy recovery (C3) and 5 % are
the examined products was captured on disposed in landfill (C4).
the basis of evaluations of internal production and
environmental data, the collection of LCA relevant data 3.9 Comparability
within the supply chain, as well as the evaluation of Basically, a comparison or an evaluation of EPD data
relevant data for the energy supply. The collected is only possible if all the data sets to be compared
data were checked for plausibility and consistency. were created according to EN 15804 and the building
Good representativity can be assumed. context, respectively the product-specific
characteristics of performance, are taken into account.
For the assessment of the variability of the results, all
products were balanced in addition to the average The background database used is GaBi 10.6 in the
database version 2021.2
4. LCA: Scenarios and additional technical information
Characteristic product properties The following technical information is a basis for the
Information on biogenic carbon declared modules.
Transport to the building site (A4)
Information on describing the biogenic Carbon Name Value Unit
Content at factory gate Transport distance (Truck) 607 km
The biogenic carbon content was calculated based on Capacity utilisation (including
55 %
the factors from the Thünen Intitute. empty runs) (Truck)
Name Value Unit Transport distance (Container
1701 km
Biogenic carbon content in Ship)
0.61 kg C
accompanying packaging Capacity utilisation (Container
80 %
Ship)
6 Environmental Product Declaration Hansgrohe Group – Showerpipes
Installation into the building (A5)
For the installation are required screws, dowels,
silicone, teflon tape and electricity for a drilling
machine. The packaging is disposed either by
recycling or incineration.
Name Value Unit
(Paper, cardboard and plastic)
1.861 kg
Packaging
Electricity consumption 0.002 kWh
Screws 0.01 kg
Dowels 0.007 kg
Silicone 0.03 kg
Teflon tape 0.1 m
Maintenance (B2)
For module B2, it is assumed that a weekly cleaning
of the product takes place, with 0.5 liter of water
containing 1.5% soap.
Name Value Unit
Number/R
Maintenance cycle (cleaning) 1040
SL
Water consumption/Cycle weekly
0.5 Liter/cycle
(cleaning)
Soap concentration (cleaning) 1.5 %
Water consumption (cleaning) 0.52 m3
Auxiliary Soap/Tensides
7.8 kg
(cleaning)
Service life
Hansgrohe SE declares a Service Life of 20 years as
an empirical value for the showerpipes when used in
accordance with the care instructions. This value is
based on their technical service centre's statistics on
service life in the market and complaints.
Name Value Unit
Life Span according to the
20 a
manufacturer
Operational energy use (B6) and Operational water
use (B7)
Name Value Unit
Water consumption 96 m3
Energy demand 4468 kWh
End of life (C1-C4)
Name Value Unit
Collected separately 4.87 kg
Recycling 3.285 kg
Energy recovery 1.347 kg
Landfilling 0.244 kg
Reuse, recovery and/or recycling potentials (D),
relevant scenario information
The energy generated from energy recovery as well as
recycled materials are assigned to module D as
possible potentials or avoided loads in subsequent
systems. Credits are only given for the primary portion
of the inputs.
7 Environmental Product Declaration Hansgrohe Group – Showerpipes
5. LCA: Results
The following table shows the result of the LCA for 1 piece of an average shower pipe. The results in the B-
module are based on a lifetime of 20 years. Scenario B6/1 shows the result for the use of a gas low temperature
boiler. Scenario B6/2 shows the result for the use of an electric instantaneous water heater.
DESCRIPTION OF THE SYSTEM BOUNDARY (X = INCLUDED IN LCA; ND = MODULE OR INDICATOR NOT
DECLARED; MNR = MODULE NOT RELEVANT)
BENEFITS AND
CONSTRUCTI LOADS
PRODUCT STAGE ON PROCESS USE STAGE END OF LIFE STAGE BEYOND THE
STAGE SYSTEM
BOUNDARIES
8 Environmental Product Declaration Hansgrohe Group – Showerpipes
lairetam
waR
ylppus tropsnarT
gnirutcafunaM
eht
morf
tropsnarT
etis
eht
ot
etag
ylbmessA esU
ecnanetniaM
riapeR
tnemecalpeR tnemhsibrufeR
ygrene
lanoitarepO esu
retaw
lanoitarepO esu
noitcurtsnoc-eD
noitilomed tropsnarT
gnissecorp
etsaW
lasopsiD -esueR -yrevoceR -gnilcyceR laitnetop
A1 A2 A3 A4 A5 B1 B2 B3 B4 B5 B6 B7 C1 C2 C3 C4 D
X X X X X X X X X X X X X X X X X
RESULTS OF THE LCA - ENVIRONMENTAL IMPACT according to EN 15804+A2: 1 piece average
showerpipe incl. packaging
Core Indicator Unit A1-A3 A4 A5 B1 B2 B3 B4 B5 B6/1 B6/2 B7 C1 C2 C3 C4 D
-
1.60E+4.45E-2.68E+0.00E+2.56E+0.00E+0.00E+0.00E+1.19E+1.78E+5.69E+0.00E+8.31E-2.66E+1.30E-
GWP-total [kg CO2-Eq.]
1 1 0 0 1 0 0 0 3 3 1 0 2 0 2
9.54E+
0
-
1.82E+4.42E- 4.27E-0.00E+1.96E+0.00E+0.00E+0.00E+1.19E+1.78E+5.69E+0.00E+8.24E-2.66E+1.30E-
GWP-fossil [kg CO2-Eq.]
1 1 1 0 1 0 0 0 3 3 1 0 2 0 2
7.39E+
0
- -
0.00E+2.25E+0.00E+0.00E+0.00E+0.00E+0.00E+0.00E+0.00E+0.00E+0.00E+0.00E+0.00E+0.00E+
GWP-biogenic [kg CO2-Eq.] 2.25E+
0 0 0 0 0 0 0 0 0 0 0 0 0 0
2.13E+
0 0
3.82E- 2.84E- 6.92E-0.00E+6.02E+0.00E+0.00E+0.00E+6.04E-2.51E+4.60E-0.00E+6.76E- 3.65E- 1.25E--2.26E-
GWP-luluc [kg CO2-Eq.]
2 3 4 0 0 0 0 0 2 0 2 0 4 4 5 2
5.24E- 7.84E- 3.12E-0.00E+1.09E-0.00E+0.00E+0.00E+4.30E- 4.25E- 5.38E-0.00E+1.63E- 7.42E- 3.09E--9.65E-
ODP [kg CFC11-Eq.]
8 17 15 0 6 0 0 0 13 11 13 0 17 10 17 8
1.83E- 4.12E- 1.15E-0.00E+6.64E-0.00E+0.00E+0.00E+7.32E-3.70E+1.40E-0.00E+1.38E- 9.67E- 4.09E--8.64E-
AP [mol H+-Eq.]
1 3 3 0 2 0 0 0 1 0 1 0 4 4 5 2
1.06E- 1.05E- 7.49E-0.00E+5.81E-0.00E+0.00E+0.00E+1.09E- 4.76E- 6.05E-0.00E+2.46E- 5.29E- 7.45E--7.36E-
EP-freshwater [kg P-Eq.]
3 6 7 0 4 0 0 0 4 3 2 0 7 7 7 4
2.22E- 1.16E- 2.52E-0.00E+1.51E-0.00E+0.00E+0.00E+3.11E- 8.78E- 2.65E-0.00E+5.44E- 3.73E- 1.01E--1.04E-
EP-marine [kg N-Eq.]
2 3 4 0 2 0 0 0 1 1 1 0 5 4 5 2
2.35E- 1.29E- 2.80E-0.00E+1.81E-0.00E+0.00E+0.00E+3.40E+9.22E+4.18E-0.00E+6.22E- 4.52E- 1.09E--1.11E-
EP-terrestrial [mol N-Eq.]
1 2 3 0 1 0 0 0 0 0 1 0 4 3 4 1
6.48E- 3.13E- 8.09E-0.00E+6.04E-0.00E+0.00E+0.00E+9.08E-2.38E+1.07E-0.00E+1.23E- 9.89E- 3.17E--3.10E-
POCP [kg NMVOC-Eq.]
2 3 4 0 2 0 0 0 1 0 1 0 4 4 5 2
6.69E- 3.37E- 5.67E-0.00E+2.11E-0.00E+0.00E+0.00E+6.41E- 5.23E- 7.41E-0.00E+7.33E- 5.06E- 8.94E--5.25E-
ADPE [kg Sb-Eq.]
3 8 6 0 5 0 0 0 5 4 6 0 9 8 10 3
-
2.77E+5.79E+5.51E+0.00E+4.52E+0.00E+0.00E+0.00E+2.05E+3.16E+5.85E+0.00E+1.10E+2.78E+1.88E-
ADPF [MJ] 8.71E+
2 0 0 0 2 0 0 0 4 4 2 0 0 0 1
1
-
[m³ world-Eq 2.12E+3.37E- 1.15E-0.00E+6.93E+0.00E+0.00E+0.00E+3.13E+2.85E+1.75E+0.00E+7.67E- 2.79E--1.41E-
WDP 1.57E+
deprived] 1 3 1 0 0 0 0 0 0 2 1 0 4 1 4
1
GWP = Global warming potential; ODP = Depletion potential of the stratospheric ozone layer; AP = Acidification potential of land and water; EP =
Caption Eutrophication potential; POCP = Formation potential of tropospheric ozone photochemical oxidants; ADPE = Abiotic depletion potential for non-
fossil resources; ADPF = Abiotic depletion potential for fossil resources; WDP = Water (user) deprivation potential
RESULTS OF THE LCA - INDICATORS TO DESCRIBE RESOURCE USE according to EN 15804+A2: 1 piece
average showerpipe incl. packaging
Indicator Unit A1-A3 A4 A5 B1 B2 B3 B4 B5 B6/1 B6/2 B7 C1 C2 C3 C4 D
-
PERE [MJ] 3.03E+12.70E-13.35E+10.00E+09.36E+10.00E+00.00E+00.00E+01.79E+21.46E+41.72E+20.00E+06.34E-29.92E-11.37E-2
5.85E+1
- -
PERM [MJ] 3.15E+10.00E+0 0.00E+00.00E+00.00E+00.00E+00.00E+0 0.00E+00.00E+00.00E+00.00E+00.00E+00.00E+00.00E+0
3.15E+1 1.00E+0
-
PERT [MJ] 6.18E+12.70E-12.03E+00.00E+09.36E+10.00E+00.00E+00.00E+01.78E+21.46E+41.72E+20.00E+06.34E-29.92E-11.37E-2
5.85E+1
-
PENRE [MJ] 2.49E+25.81E+07.82E+00.00E+04.52E+20.00E+00.00E+00.00E+02.05E+43.16E+45.86E+20.00E+01.11E+02.76E+11.50E+0
8.74E+1
- - - -
PENRM [MJ] 2.85E+10.00E+0 0.00E+00.00E+00.00E+00.00E+00.00E+0 0.00E+00.00E+00.00E+00.00E+0 0.00E+0
2.31E+0 1.00E+0 2.48E+11.31E+0
-
PENRT [MJ] 2.77E+25.81E+05.51E+00.00E+04.52E+20.00E+00.00E+00.00E+02.05E+43.16E+45.86E+20.00E+01.11E+02.78E+01.88E-1
8.74E+1
SM [kg] 2.26E+00.00E+00.00E+00.00E+00.00E+00.00E+00.00E+00.00E+00.00E+00.00E+00.00E+00.00E+00.00E+00.00E+00.00E+03.03E+0
4.12E- -8.59E-
RSF [MJ] 0.00E+00.00E+00.00E+00.00E+00.00E+00.00E+00.00E+00.00E+00.00E+00.00E+00.00E+00.00E+00.00E+00.00E+0
23 23
NRSF [MJ] 0.00E+00.00E+00.00E+00.00E+00.00E+00.00E+00.00E+00.00E+00.00E+00.00E+00.00E+00.00E+00.00E+00.00E+00.00E+00.00E+0
FW [m³] 5.16E-13.11E-43.72E-30.00E+01.62E-10.00E+00.00E+00.00E+02.00E-11.42E+14.99E-10.00E+07.26E-56.95E-32.25E-6-3.60E-1
PERE = Use of renewable primary energy excluding renewable primary energy resources used as raw materials; PERM = Use of
renewable primary energy resources used as raw materials; PERT = Total use of renewable primary energy resources; PENRE = Use of
non-renewable primary energy excluding non-renewable primary energy resources used as raw materials; PENRM = Use of non-
Caption
renewable primary energy resources used as raw materials; PENRT = Total use of non-renewable primary energy resources; SM = Use
of secondary material; RSF = Use of renewable secondary fuels; NRSF = Use of non-renewable secondary fuels; FW = Use of net fresh
water
RESULTS OF THE LCA – WASTE CATEGORIES AND OUTPUT FLOWS according to EN 15804+A2:
1 piece average showerpipe incl. packaging
Indicator Unit A1-A3 A4 A5 B1 B2 B3 B4 B5 B6/1 B6/2 B7 C1 C2 C3 C4 D
2.54E- 5.82E- 6.57E- 3.34E-
HWD [kg] 1.15E-5 3.78E-90.00E+08.50E-30.00E+00.00E+00.00E+03.83E-68.35E-61.20E-70.00E+0 -5.19E-5
10 11 10 11
-
NHWD [kg] 2.70E+08.45E-46.36E-20.00E+06.58E-10.00E+00.00E+00.00E+02.69E+02.24E+19.35E+10.00E+01.73E-41.54E-12.44E-1
1.87E+0
RWD [kg] 7.39E-39.72E-62.34E-40.00E+04.13E-30.00E+00.00E+00.00E+04.52E-24.71E+04.81E-20.00E+02.01E-61.45E-42.16E-6-3.28E-3
CRU [kg] 0.00E+00.00E+00.00E+00.00E+00.00E+00.00E+00.00E+00.00E+00.00E+00.00E+00.00E+00.00E+00.00E+00.00E+00.00E+00.00E+0
MFR [kg] 0.00E+00.00E+01.67E+00.00E+00.00E+00.00E+00.00E+00.00E+00.00E+00.00E+00.00E+00.00E+00.00E+03.29E+00.00E+00.00E+0
MER [kg] 0.00E+00.00E+00.00E+00.00E+00.00E+00.00E+00.00E+00.00E+00.00E+00.00E+00.00E+00.00E+00.00E+00.00E+00.00E+00.00E+0
EEE [MJ] 2.85E-10.00E+05.20E-10.00E+00.00E+00.00E+00.00E+00.00E+00.00E+00.00E+00.00E+00.00E+00.00E+02.88E-22.90E-40.00E+0
EET [MJ] 6.16E-10.00E+09.38E-10.00E+00.00E+00.00E+00.00E+00.00E+00.00E+00.00E+00.00E+00.00E+00.00E+05.41E-20.00E+00.00E+0
HWD = Hazardous waste disposed; NHWD = Non-hazardous waste disposed; RWD = Radioactive waste disposed; CRU = Components
Caption for re-use; MFR = Materials for recycling; MER = Materials for energy recovery; EEE = Exported electrical energy; EET = Exported
thermal energy
RESULTS OF THE LCA – additional impact categories according to EN 15804+A2-optional:
1 piece average showerpipe incl. packaging
Indicator Unit A1-A3 A4 A5 B1 B2 B3 B4 B5 B6/1 B6/2 B7 C1 C2 C3 C4 D
[Disease 0.00E+ 0.00E+ 0.00E+ 0.00E+ 0.00E+ 8.64E- 4.33E- -8.96E-
PM 1.67E-66.41E-81.31E-8 3.31E-6 5.08E-63.12E-51.57E-6 9.00E-9
Incidence] 0 0 0 0 0 10 10 7
-
[kBq U235- 3.37E+ 0.00E+ 2.14E+ 0.00E+ 0.00E+ 0.00E+ 7.19E+ 7.72E+ 7.57E+ 0.00E+
IRP 1.42E-33.52E-2 2.93E-41.41E-23.09E-41.92E+
Eq.] 0 0 0 0 0 0 0 2 0 0
0
-
1.42E+ 4.27E+ 2.18E+ 0.00E+ 2.00E+ 0.00E+ 0.00E+ 0.00E+ 2.80E+ 1.33E+ 8.26E+ 0.00E+ 2.48E+
ETP-fw [CTUe] 8.17E-1 9.38E-21.66E+
3 0 0 0 2 0 0 0 2 4 3 0 0
2
8.51E- 0.00E+ 0.00E+ 0.00E+ 0.00E+ 0.00E+ 1.65E- 7.00E- 6.99E- -1.92E-
HTP-c [CTUh] 4.39E-7 1.66E-8 2.21E-8 5.99E-83.76E-72.81E-7
11 0 0 0 0 0 11 11 12 8
0.00E+ 0.00E+ 0.00E+ 0.00E+ 0.00E+ 8.79E- 6.63E- -5.28E-
HTP-nc [CTUh] 1.96E-64.42E-91.28E-7 7.49E-7 6.32E-61.42E-52.89E-5 6.33E-9
0 0 0 0 0 10 10 7
-
1.09E+ 1.59E+ 7.40E+ 0.00E+ 3.18E+ 0.00E+ 0.00E+ 0.00E+ 1.19E+ 9.97E+ 2.89E+ 0.00E+
SQP [-] 3.79E-18.65E-11.37E-22.73E+
2 0 0 0 2 0 0 0 2 3 2 0
2
PM = Potential incidence of disease due to PM emissions; IR = Potential Human exposure efficiency relative to U235; ETP-fw = Potential
Caption comparative Toxic Unit for ecosystems; HTP-c = Potential comparative Toxic Unit for humans (cancerogenic); HTP-nc = Potential
comparative Toxic Unit for humans (not cancerogenic); SQP = Potential soil quality index
Disclaimer 1 – for the indicator “Potential Human exposure efficiency relative to U235”.
This impact category deals mainly with the eventual impact of low dose ionizing
radiation on human health of the nuclear fuel cycle. It does not consider effects due to possible
nuclear accidents, occupational exposure nor due to radioactive waste disposal in underground
facilities. Potential ionizing radiation from the soil, from radon and from some construction materials is also not
measured by this indicator.
Disclaimer 2 – for the indicators “abiotic depletion potential for non-fossil resources”, “abiotic depletion potential
for fossil resources”, “water (user) deprivation potential, deprivation-weighted water consumption”, “potential
comparative toxic unit for ecosystems”, “potential comparative toxic unit for humans – cancerogenic”, “Potential
comparative toxic unit for humans - not cancerogenic”, “potential soil quality index”.
The results of this environmental impact indicator shall be used with care as the
uncertainties on these results are high or as there is limited experienced with the indicator.
6. LCA: Interpretation
9 Environmental Product Declaration Hansgrohe Group – Showerpipes
The dominance analysis shows that modules B2, B6 an influence on construction and materials used. The
and B7 are the dominant life cycle stages in most of basic structure of the product types is always similar.
the categories. The contribution of B2 is due to the Material type and quantity proportions do not differ
demand of soap and water for cleaning. Module B6 much, as also shown in the average material
dominates most of the indicators due to the energy composition table.
demand for water heating and module B7 has a high The deviation of the GWP fossil in modules A1-C4 has
contribution to EPfreshwater due to the wastewater a maximum of 55% and a minimum of -49% with
treatment. The module A1-A3 has a very low scenario B6/1 (gas low temperature boiler). The
contribution to all categories except of ADPE. In this deviation of the GWP fossil in modules A1-C4 has a
indicator the provision of brass has the largest maximum of 55% and a minimum of -50% with
contribution. The end-of-life stage has no significant scenario B6/2 (electric instantaneous water heater).
influence on the environmental indicators. For an average scenario, where 50% of water is
The environmental burdens from the transports heated with gas low temperature boiler and 50% with
(modules A4 and C2) account for less than 1% of the electric instantaneous water heater, 66% of the shower
total burdens of the respective indicators in all cases. pipes produced are above the average GWP fossil
The possible potentials of avoided loads of subsequent value. Whereas 34% reflect the average or are lower
systems (module D) lie outside the considered system than the average. However, 82% of the ones which are
boundaries and relate exclusively to credits from above the average just deviate between +1 and +17
recycling and thermal recycling by means of %.
incineration with energy recovery of the different Modules B6 and B7 account for more than 90% of the
materials. GWP indicator. The deviation from the average is
986,466 showerpipes of 150 different product types mainly caused by the flow rate in module B7. The
were produced. For the assessment of the variability of higher the deviation from the average GWP, the higher
the results, all products were balanced and compared the flow rate. The flow rate ranges between 6.6 and
to the average product weighted by production volume. 21.2 l/min. Consequently, the production phase has a
The different types of products all have the same minor influence on the LCA results.
function and differ mainly in terms of design, which has
7. Requisite evidence
The drinking water regulation determines the quality of - Part A – Procedure for the acceptance
drinking water at the point of withdrawal. This result in - Part B – 4MS Common Composition List
requirements for used materials in drinking water  Metal recommendation of the federal
installations in general and therefore in sanitary fittings environment agency: metal materials suitable
in particular.
for drinking water hygiene
All materials used by Hansgrohe SE, which are in
contact with drinking water, fulfill the drinking water
regulation. Regulations for other materials (Germany):
Regulations for metals (Europe-wide):  KTW: Assessment basis for plastics and other
 Acceptance of metallic materials used for organic materials in contact with drinking
products in contact with drinking water: 4MS water
Common Approach  Elastomer guideline: Guideline for the
10 Environmental Product Declaration Hansgrohe Group – Showerpipes
hygienic assessment of elastomers in contact drinking water (sanitary lubricants), (Lubricant
with drinking water Guideline)
 Thermoplastic elastomers: Recommendation
for the hygienic assessment of products made Regulation for other materials (France):
of thermoplastic elastomers in contact with  ACS: Attestation de Conformité Sanitaire
drinking water (TPE transition (plastics, elastomers, metals)
recommendation)
 Ceramics: draft assessment basis for Regulation for other materials (UK):
enamels and ceramic materials: assessment  BS 69 20: Suitability of non-metallic products
basis for enamels and ceramic materials in for use in contact with water intended for
contact with drinking water (enamel/ceramic human consumption with regard to their effect
assessment basis) on the quality of water (plastics, elastomers)
 Lubricants: Guideline for the hygienic
assessment of lubricants in contact with Products of the Hansgrohe SE are therefore uncritical
to use with any drinking water.
8. References
Standards DIN EN ISO 14001
DIN EN ISO 14001:2015, Environmental management
EN 200 systems — Requirements with guidance for use, 2015-
EN 200:2008: Sanitary tapware – Single taps and 09
combination taps for water supply systems of type 1
and type 2 DIN EN ISO 14025
DIN EN ISO 14025: Environmental labels and
EN 816 declarations - Type III environmental declarations -
EN 816:2017: Sanitary tapware – Automatic shut-off Principles and procedures, 2011-10
valves PN 10
EN 15804
EN 817 DIN EN 15804:2012+A2:2019+AC:2021: Sustainability
EN 817:2008: Sanitary tapware – Mechanical mixing of construction works - Environmental product
valves (PN 10) declarations - Core rules for the product category of
construction products
EN 1111
EN 1111:2018: Sanitary tapware – Thermostatic DIN EN ISO 45001
mixing valves (PN 10) DIN EN ISO 45001:2018: Occupational health and
safety management systems — Requirements with
EN 1112 guidance for use. 2018-03
EN 1112:2008 Sanitary tapware - Shower outlets for
sanitary tapware for water supply systems of type 1 DIN EN ISO 50001
and type 2 - General technical specification DIN EN ISO 50001:2018: Energy management
systems — Requirements with guidance for use. 2018-
EN 1113 08
EN 1113:2015 Sanitary tapware – Shower hoses for
sanitary tapware for water supply systems of type 1 Further References
and type 2 - General technical specification
AVV
ISO 3822 Draft General administrative provision relating to the
ISO 3822: Acoustics – Laboratory tests on noise Order on the European list of wastes (Waste List Order
emission from appliances and equipment used in water – German designation: AVV) of 10 December 2001.
supply installations
ECHA
DIN 4102-1 European Chemicals Agency (ECHA) Candidate List of
DIN 4102-1: Fire behaviour of building materials and Substances of Very High Concern (SVHC) for
building components - Part 1: Building materials; Authorisation https://echa.europa.eu/de/candidate-
concepts, requirements and tests. 1998-05 listtable
DIN EN ISO 9001 Ecoinvent
DIN EN ISO 9001:2015: Quality management systems ecoinvent 3.6 Database on Life Cycle Inventories (Life
- Requirements (ISO 9001:2015) Cycle Inventory data), ecoinvent Association, Zürich,
2020
DIN EN 13501-1
DIN EN 13501-1:2019-05: Fire classification of EU Ordinance on biocide Products No. 528/2012
construction products and building elements - Part 1: European Parliament, 2012. Regulation (EU) no
Classification using data from reaction to fire tests; 528/2012 of the European parliament and of the
German version EN 13501-1:2018 council of 22 May 2012 concerning the making
available on the market and use of biocidal products
11 Environmental Product Declaration Hansgrohe Group – Showerpipes
Services. Part A: Calculation rules for the life cycle
Eurostat assessment and requirements on the project report.
Eurostat, last update 26/10/2021 on Version 2.1, Berlin, 11/2021
https://ec.europa.eu/eurostat/databrowser/view/ten000
63/default/table?lang=en PCR Part B
Institut Bauen und Umwelt e.V. (IBU), Requirements
GaBi on the EPD for fittings and showers. Version 1.1,
GaBi 10.6, GaBi Software System and Database for Berlin, 03/2022
Life Cycle Engineering version 2021.2, Sphera
Solutions GmbH, Leinfelden-Echterdingen, 1992-2021 Thünen Institute
Diestel, Sylvia / Weimar, Holger: Der Kohlenstoffgehalt
IBU 2021 in Holz- und Papierprodukten - Herleitung und
General Instructions for the EPD programme of Institut Umrechnungsfaktoren. Thünen Working Paper 38.
Bauen und Umwelt e.V. Version 2.0, Berlin: Institut Johann Heinrich von Thünen-Institut. Hamburg, 2014
Bauen und Umwelt e.V., 2021, www.ibu-epd.com
PCR Part A
Institut Bauen und Umwelt e.V. (IBU), Product
Category Rules for Building-Related Products and
12 Environmental Product Declaration Hansgrohe Group – Showerpipes
Publisher
Institut Bauen und Umwelt e.V. Tel +49 (0)30 3087748- 0
Hegelplatz 1 Fax +49 (0)30 3087748- 29
10117 Berlin Mail info@ibu-epd.com
Germany Web www.ibu-epd.com
Programme holder
Institut Bauen und Umwelt e.V. Tel +49 (0)30 - 3087748- 0
Hegelplatz 1 Fax +49 (0)30 – 3087748 - 29
10117 Berlin Mail info@ibu-epd.com
Germany Web www.ibu-epd.com
Author of the Life Cycle
Assessment Tel +49 421 70 90 84 33
brands & values GmbH Fax +49 421 70 90 84 35
Altenwall 14 Mail info@brandsandvalues.com
28195 Bremen Web www.brandsandvalues.com
Germany
Owner of the Declaration
Hansgrohe Group Tel +49 7836 51-0
Auestr. 5-9 Fax +49 7836 51-1300
77761 Schiltach Mail info@hansgrohe-group.com
Germany Web http://www.hansgrohe-
group.com
