ENVIRONMENTAL PRODUCT DECLARATION
as per ISO 14025 and EN 15804+A2
Owner of the Declaration VELUX Group
Publisher Institut Bauen und Umwelt e.V. (IBU)
Programme holder Institut Bauen und Umwelt e.V. (IBU)
Declaration number EPD-VEL-20230506-CBA1-EN
Issue date 11/03/2024
Valid to 10/03/2029
VELUX insulated installation frame BGX
VELUX A/S
www.ibu-epd.com | https://epd-online.com
General Information
VELUX A/S VELUX insulated installation frame BGX
Programme holder Owner of the declaration
IBU – Institut Bauen und Umwelt e.V. VELUX Group
Hegelplatz 1 Ådalsvej 99
10117 Berlin 2970 Hørsholm
Germany Denmark
Declaration number Declared product / declared unit
EPD-VEL-20230506-CBA1-EN 1m² insulated installation frame BGX.
The declared unit is based on the configuration of a standard size window
measuring 1.34 m x 1.60 m.
(The declared representative product of the product group comprise the
product with the highest mass.)
This declaration is based on the product category rules: Scope:
Windows and doors , 01/08/2021 Productline BGX - insulated installation frame; manufactured by VELUX in
(PCR checked and approved by the SVR) Poland for sale in Europe.
Declaration according to ISO 14025 and EN 15804 describing specific
Issue date environmental performance of the construction product.
11/03/2024
The owner of the declaration shall be liable for the underlying information
and evidence; the IBU shall not be liable with respect to manufacturer
information, life cycle assessment data and evidences.
Valid to
10/03/2029 The EPD was created according to the specifications of EN 15804+A2. In
the following, the standard will be simplified as EN 15804.
Verification
The standard EN 15804 serves as the core PCR
Independent verification of the declaration and data according to ISO
14025:2011
internally X externally
Dipl.-Ing. Hans Peters
(Chairman of Institut Bauen und Umwelt e.V.)
Florian Pronold Dr.-Ing. Nikolay Minkov,
(Managing Director Institut Bauen und Umwelt e.V.) (Independent verifier)
1 Environmental Product Declaration - VELUX A/S - VELUX insulated installation frame BGX
Product
specifications and test methods/test standards can be
Product description/Product definition downloaded from the website www.velux.com/ce-marking.
Insulated installation frame BGX consists of four bars of
Purenit® sandwich foam, joined to form a frame in which a roof The performance values are specific for the BGX insulated
window can be installed. installation frame.
Insulated installation frame BGX is especially designed for The declared values in the table relate to the reference product.
installation in warm roof constructions with solid insulation. BGX For other covered product variants, specific values can be
fits counter battens and battens with a thickness of 40 mm and selected at the bottom of the above-mentioned download page.
30 mm respectively. BGX ensures that the window is fastened
Constructional data
securely to the roof construction, provides optimum insulation
and also wind and watertight connection. Name Value Unit
Reaction to fire E class
Insulated installation frame BGX is available for single roof Thermal resistance 0.044 W/(mK)
windows only, but by adding extension bars BGX WK--, the
Durability No performance determined
installation frame can be used when installing additional
elements GIL/GIU (WK34) and VELUX CABRIO® roof balcony Performance data of the product in accordance with the
GDL (WK19) as well. declaration of performance with respect to its essential
characteristics according to EN 13165:2012+A1:2015, Thermal
insulation products for buildings
Installation angle
Base materials/Ancillary materials
The insulation product can be installed within the roof pitch
from 15° to 90°. Name Value Unit
Plastics 95.9 %
For the placing on the market of the product in the European Steel 4.1 %
Union/European Free Trade Association (EU/EFTA) (with the
REACH
exception of Switzerland) Regulation (EU) No. 305/2011 (CPR)
This product contains substances listed in the candidate list
applies. The product needs a declaration of performance taking
(date: 09.08.2023) exceeding 0.1 percentage by mass: no.
into consideration EN 13165:2012+A1:2015, Thermal insulation
products for buildings and the CE-marking.
Reference service life
A calculation of the reference service life according to ISO
15686 is not possible.
For the application and use the respective national provisions
apply.
The Bundesinstitut für Bau, Stadt und Raumforschung/Federal
Application office for building and regional planning (BBSR) table declares
for the complete roof window a service life dependent on the
Insulated installation frame BGX is especially designed for
applied window frame material between 25 and ≥ 50 years.
installation in warm roof constructions with solid insulation.
This includes insulated installation frames as declared with this
Technical Data EPD.
The Declaration of Performance including relevant technical
LCA: Calculation rules
Type of EPD: Cradle to gate - with options. The following life
Declared Unit cycle stages were considered:
The declared unit is 1 m² related to a reference window, that
the insulated installation frame is installed in connection with. Production stage A1-A3:
The declared unit is based on the representative product Consideration of the production of raw materials (PU-foam
measuring 1.34 m x 1.60 m. profile, plastics and steel) and their processing (estimated
The product BGX is manufactured in Poland. energy data: electrical energy from the national residual mix
Declared unit and mass reference and thermal energy from natural gas); transport of major
materials to the manufacturing site; assembly of semi-finished
Name Value Unit
products to the final product; packaging material (including
Declared unit 1 m2 waste paper input for paper and cardboard).
Grammage 6.21 kg/m2
Layer thickness 0 m End-of-Life stage C1, C2, C3:
C1: a manual demolition is assumed, resulting in indicator value
Weight per area 13.31 kg/representative product
"0".
Weight per area 6.21 kg/declared unit
C2: For the transport to EoL by truck a distance of 50 km is
assumed.
The calculation is based mainly on BOM (Bill of Materials) data, C3: A scenario for the incineration of plastics in a waste
with only a few specific information on processing. This may incineration plant (WIP) is assumed; metals are assumed to be
lead to a higher uncertainty for the result values and needs to recycled.
be kept in mind for the application of this EPD.
System boundary The EoL-Scenario does not assume waste to be disposed of on
2 Environmental Product Declaration - VELUX A/S - VELUX insulated installation frame BGX
a landfill site. Module C4 is declared as"0".
Geographic Representativeness
Benefits for the next product system D: Land or region, in which the declared product system is
Resulting electrical and thermal energy from the WIP, avoiding manufactured, used or handled at the end of the product´s
the generation of electricity and heat via fossil fuels, is lifespan: Europe
considered.
The amount of metals after the reduction due to the net-flow
Comparability
calculations is sent to a recycling process. The effort for
Basically, a comparison or an evaluation of EPD data is only
recycling, as well as the benefit for the regained metals are
possible if all the data sets to be compared were created
declared in module D.
according to EN 15804 and the building context, respectively
the product-specific characteristics of performance, are taken
Contribution of waste flows is considered in the modules where
into account. The software LCA FE 10.7 is used accompanied
they occur.
by the MLC database (version 2023.1, 2023).
LCA: Scenarios and additional technical information
Characteristic product properties of biogenic carbon
The following declared values refer to the declared unit of 1m².
Information on describing the biogenic carbon content at
factory gate
The declared biogenic content comprises the paper manual
and the packaging material consisting of cardboard, paper, PE Reference service life
and EPS. As module A5 is not declared, the information on Name Value Unit
packaging supports further EoL calculations.
Life Span (according to BBSR) 25 - 50 a
Name ValueUnit
kg End of life (C1-C4)
Biogenic carbon content in product -
C Name Value Unit
Biogenic carbon content in accompanying kg Collected separately waste type 6.21 kg
0.3
packaging C Recycling 0.25 kg
The value refers to the following packaging material (per 1m²): Energy recovery 5.95 kg
Paper (manual): 0.009 kg,
Cardboard packaging: 0.592 kg, Reuse, recovery and/or recycling potentials (D), relevant
PE-LD: 0.014 kg, scenario information
EPS: 0.009 kg. Name Value Unit
Steel (net-flow-calculation) 0.30 kg/1m² product
Note: 1 kg of biogenic carbon is equivalent to 44/12 kg of CO .
2
3 Environmental Product Declaration - VELUX A/S - VELUX insulated installation frame BGX
LCA: Results
The LCIA assessment is performed applying the characterisation factors "EN 15804+A2, EF 3.0".
DESCRIPTION OF THE SYSTEM BOUNDARY (X = INCLUDED IN LCA; MND = MODULE OR INDICATOR NOT DECLARED; MNR
= MODULE NOT RELEVANT)
Benefits and
Construction loads beyond
Product stage Use stage End of life stage
process stage the system
boundaries
la ire ta m w a Ry lp p u s tro p s n a rT g n iru tc a fu n a M e h t m o rf tro p s n a rTe tis e h t o t e ta g y lb m e s s A e s U e c n a n e tn ia M ria p e R tn e m e c a lp e R tn e m h s ib ru fe R y g re n e la n o ita re p Oe s u re ta w la n o ita re p Oe s u n o itc u rts n o c -e Dn o itilo m e d tro p s n a rT g n is s e c o rp e ts a W la s o p s iD -e s u e R-y re v o c e R-g n ilc y c e Rla itn e to p
A1 A2 A3 A4 A5 B1 B2 B3 B4 B5 B6 B7 C1 C2 C3 C4 D
X X X MND MND MND MND MNR MNR MNR MND MND X X X X X
RESULTS OF THE LCA - ENVIRONMENTAL IMPACT according to EN 15804+A2: 1 m² insulated installation frame BGX
Parameter Unit A1-A3 C1 C2 C3 C4 D
Global Warming Potential total (GWP-total) kg CO 2 eq 2.12E+01 0 2.39E-02 1.34E+01 0 -3.23E+00
Global Warming Potential fossil fuels (GWP-fossil) kg CO 2 eq 2.12E+01 0 2.27E-02 1.34E+01 0 -3.22E+00
Global Warming Potential biogenic (GWP-biogenic) kg CO 2 eq -6.19E-02 0 9.95E-04 9.3E-04 0 -1.51E-02
Global Warming Potential luluc (GWP-luluc) kg CO 2 eq 1.02E-02 0 2.07E-04 2.15E-05 0 -1.85E-04
Depletion potential of the stratospheric ozone layer (ODP) kg CFC11 eq 1.09E-10 0 2.91E-15 1.06E-12 0 -2.11E-11
Acidification potential of land and water (AP) mol H+ eq 3.29E-02 0 4.49E-05 7.5E-03 0 -4.46E-03
Eutrophication potential aquatic freshwater (EP-freshwater) kg P eq 7.94E-05 0 8.17E-08 2.86E-07 0 -4.45E-06
Eutrophication potential aquatic marine (EP-marine) kg N eq 1.03E-02 0 1.85E-05 3.62E-03 0 -1.17E-03
Eutrophication potential terrestrial (EP-terrestrial) mol N eq 1.09E-01 0 2.11E-04 4.18E-02 0 -1.22E-02
Formation potential of tropospheric ozone photochemical oxidants kg NMVOC
4.34E-02 0 4.01E-05 9.29E-03 0 -3.52E-03
(POCP) eq
Abiotic depletion potential for non fossil resources (ADPE) kg Sb eq 6.54E-06 0 1.47E-09 1.01E-08 0 -1.48E-06
Abiotic depletion potential for fossil resources (ADPF) MJ 4.2E+02 0 3.04E-01 3.43E+00 0 -5.41E+01
m3 world eq
Water use (WDP) 1.71E+00 0 2.7E-04 1.31E+00 0 -3.52E-01
deprived
RESULTS OF THE LCA - INDICATORS TO DESCRIBE RESOURCE USE according to EN 15804+A2: 1 m² insulated installation
frame BGX
Parameter Unit A1-A3 C1 C2 C3 C4 D
Renewable primary energy as energy carrier (PERE) MJ 5.87E+01 0 2.22E-02 6.66E-01 0 -1.41E+01
Renewable primary energy resources as material utilization
MJ 1.06E+00 0 0 -1.43E-02 0 0
(PERM)
Total use of renewable primary energy resources (PERT) MJ 5.98E+01 0 2.22E-02 6.52E-01 0 -1.41E+01
Non renewable primary energy as energy carrier (PENRE) MJ 3.18E+02 0 3.06E-01 8.89E+01 0 -5.41E+01
Non renewable primary energy as material utilization (PENRM) MJ 8.64E+01 0 0 -8.55E+01 0 0
Total use of non renewable primary energy resources (PENRT) MJ 4.05E+02 0 3.06E-01 3.44E+00 0 -5.41E+01
Use of secondary material (SM) kg 3.83E+00 0 0 0 0 2.98E-01
Use of renewable secondary fuels (RSF) MJ 0 0 0 0 0 0
Use of non renewable secondary fuels (NRSF) MJ 0 0 0 0 0 0
Use of net fresh water (FW) m3 1.25E-01 0 2.43E-05 3.08E-02 0 -1.39E-02
RESULTS OF THE LCA – WASTE CATEGORIES AND OUTPUT FLOWS according to EN 15804+A2:
1 m² insulated installation frame BGX
Parameter Unit A1-A3 C1 C2 C3 C4 D
Hazardous waste disposed (HWD) kg 2.2E-07 0 9.46E-13 2.96E-10 0 -2.63E-09
Non hazardous waste disposed (NHWD) kg 2.85E-01 0 4.66E-05 6.96E-02 0 4.75E-02
Radioactive waste disposed (RWD) kg 5.8E-03 0 5.72E-07 1.42E-04 0 -3.83E-03
Components for re-use (CRU) kg 0 0 0 0 0 0
Materials for recycling (MFR) kg 0 0 0 2.52E-01 0 0
Materials for energy recovery (MER) kg 0 0 0 0 0 0
Exported electrical energy (EEE) MJ 2.38E+00 0 0 2.33E+01 0 0
Exported thermal energy (EET) MJ 4.26E+00 0 0 4.17E+01 0 0
RESULTS OF THE LCA – additional impact categories according to EN 15804+A2-optional:
1 m² insulated installation frame BGX
Parameter Unit A1-A3 C1 C2 C3 C4 D
Disease
Incidence of disease due to PM emissions (PM) 1.08E-07 0 2.9E-10 2.1E-08 0 -4.41E-08
incidence
Human exposure efficiency relative to U235 (IR) kBq U235 eq 9.49E-02 0 8.53E-05 2.25E-02 0 -6.25E-01
Comparative toxic unit for ecosystems (ETP-fw) CTUe 4.7E+01 0 2.16E-01 1.17E+00 0 -1.11E+01
4 Environmental Product Declaration - VELUX A/S - VELUX insulated installation frame BGX
Comparative toxic unit for humans (carcinogenic) (HTP-c) CTUh 9.29E-10 0 4.43E-12 9.16E-11 0 -7.58E-10
Comparative toxic unit for humans (noncarcinogenic) (HTP-nc) CTUh 3.55E-08 0 2.5E-10 3.12E-09 0 -2.4E-08
Soil quality index (SQP) SQP 3.84E+01 0 1.27E-01 7.59E-01 0 -9.43E+00
Disclaimer 1 – for the indicator 'Potential Human exposure efficiency relative to U235'. This impact category deals mainly with the
eventual impact of low-dose ionizing radiation on human health of the nuclear fuel cycle. It does not consider effects due to possible
nuclear accidents, occupational exposure or radioactive waste disposal in underground facilities. Potential ionizing radiation from the
soil, radon and from some construction materials is also not measured by this indicator.
Disclaimer 2 – for the indicators 'abiotic depletion potential for non-fossil resources', 'abiotic depletion potential for fossil resources',
'water (user) deprivation potential, deprivation-weighted water consumption', 'potential comparative toxic unit for ecosystems', 'potential
comparative toxic unit for humans – cancerogenic', 'Potential comparative toxic unit for humans - not cancerogenic', 'potential soil
quality index'. The results of this environmental impact indicator shall be used with care as the uncertainties on these results are high
as there is limited experience with the indicator.
Disclaimer 3 – for 'potential soil quality index'. Due to a data lack in the foreground data of VELUX, the result has a very high
uncertainty and refers only to the background data, which contain respective information.
Disclaimer 4 – the result values of the product BGX are partly based on data for polyurethane. For this material LCIA data of
ökobau.dat are applied, which lacks the information for the additional environmental indicators. The supposed underestimated values
for the product BGX are displayed in the report, but not declared in the EPD.
References
Standards
LCA FE 10.7 / MLC DB
EN 15804 Sphera's LCA Software for Experts / Managed LCA Content
EN 15804:2012+A2:2019+AC:2021, Sustainability of database, Sphera Solutions GmbH, Leinfelden-Echterdingen,
construction works — Environmental Product Declarations — database version 2023.1, 2023
Core rules for the product category of construction products.
ökobau.dat
ISO 14025 https://www.oekobaudat.de/
EN ISO 14025:2011, Environmental labels and declarations —
Type III environmental declarations — Principles and PCR part A
procedures. Calculation Rules for the Life Cycle Assessment and
Requirements on the Project Report according to EN
ISO 15686 15804+A2:2019, version 1.3, IBU, 2022
ISO 15686-1:2011-05: Buildings and constructed assets -
Service life planning
PCR part B
Requirements on the EPD for Windows and doors, version
EN 13165 01.08.2021, IBU
EN 13165:2012+A1:2015, Thermal insulation products for
buildings - Factory made rigid polyurethane foam (PU) products REACH/candidate list
Regulation (EC) No 1907/2006: Registration, Evaluation,
Authorisation and Restriction of Chemicals (REACH)
Further References
Regulation (EU) No. 305/2011 (CPR)
BBSR Regulation (EU) No 305/2011 of the European Parliament and
BBSR, 24.02.2017, Nutzungsdauer von Bauteilen nach BNB of the
Council
IBU 2021 of 9 March 2011 laying down harmonised conditions for the
Institut Bauen und Umwelt e.V.: General Instructions for the marketing of construction products and repealing Council
EPD programme of Institut Bauen und Umwelt e.V., Version Directive 89/106/EEC Text with EEA relevance
2.0, Berlin: Institut Bauen und Umwelt e.V., 2021
www.ibu-epd.com
5 Environmental Product Declaration - VELUX A/S - VELUX insulated installation frame BGX
Publisher
Institut Bauen und Umwelt e.V. +49 (0)30 3087748- 0
Hegelplatz 1 info@ibu-epd.com
10117 Berlin www.ibu-epd.com
Germany
Programme holder
Institut Bauen und Umwelt e.V. +49 (0)30 3087748- 0
Hegelplatz 1 info@ibu-epd.com
10117 Berlin www.ibu-epd.com
Germany
Author of the Life Cycle Assessment
Angela Schindler Umweltberatung 07553 919 9456
Tüfinger Str. 12 angela@schindler-umwelt.de
88682 Salem www.schindler-umwelt.de
Germany
Daxner & Merl GmbH +43 676 849477826
Schleifmühlgasse 13/24 office@daxner-merl.com
1040 Wien www.daxner-merl.com
Austria
Owner of the Declaration
VELUX Group +4545164726
Ådalsvej 99 jakob.roerbech@velux.com
2970 Hørsholm www.velux.com
Denmark
6 Environmental Product Declaration - VELUX A/S - VELUX insulated installation frame BGX
