ENVIRONMENTAL PRODUCT DECLARATION
as per ISO 14025 and EN 15804+A1
Owner of the Declaration ArcelorMittal Commercial RPS S.à r.l.
Programme holder Institut Bauen und Umwelt e.V. (IBU)
Publisher Institut Bauen und Umwelt e.V. (IBU)
Declaration number EPD-ARM-20210178-CBD1-EN
Issue date 22.07.2021
Valid to 21.07.2026
EcoSheetPile™ Plus
ArcelorMittal
www.ibu-epd.com | https://epd-online.com
Umwelt Produktdeklaration Name des Herstellers – Name des Produkts
General Information
ArcelorMittal EcoSheetPile™ Plus
Programme holder Owner of the declaration
IBU – Institut Bauen und Umwelt e.V. ArcelorMittal Commercial RPS S.àr.l.
Panoramastr. 1 66, rue de Luxembourg
10178 Berlin L-4221 Esch-sur-Alzette
Germany Luxembourg
Declaration number Declared product / declared unit
EPD-ARM-20210178-CBD1-EN 1 metric ton of EcoSheetPile™ Plus
This declaration is based on the product Scope:
category rules: The declaration applies to 1 metric ton of
Structural steels, 11.2017 EcoSheetPile™ Plus. It covers hot rolled steel sheet
(PCR checked and approved by the SVR) piles (Z-shaped, U-shaped, straight-web, and H-
shaped) produced by ArcelorMittal .
Issue date
22.07.2021 This environmental product declaration is valid for steel
sheet piles produced by ArcelorMittal sites Differdange
and Esch-Belval in Luxembourg. The data used
Valid to
represent 100% of the annual production of 2019 and
21.07.2026
is based on 2019 data for deliveries based on
Guarantee of Origins for 100% renewable electricity
supply.
The owner of the declaration shall be liable for the
underlying information and evidence; the IBU shall not
be liable with respect to manufacturer information, life
cycle assessment data and evidences.
The EPD was created according to the specifications
of EN 15804+A1. In the following, the standard will be
simplified as EN 15804.
Verification
The standard EN 15804 serves as the core PCR
Independent verification of the declaration and data
according to ISO 14025:2010
Dipl. Ing. Hans Peters internally x externally
(chairman of Institut Bauen und Umwelt e.V.)
Dr. Alexander Röder Matthias Klingler
(Managing Director Institut Bauen und Umwelt e.V.)) (Independent verifier)
Product
Product description/Product definition For the use and application of the product the
This EPD applies to 1 metric ton of steel sheet piles respective national provisions at the place of use
EcoSheetPile™ Plus in steel grades EN 10248-1 - apply, in Germany for example the building codes of
S 240 GP to S 355 GP, ASTM A572 - Gr.50 and CSA the federal states and the corresponding national
350W for civil engineering applications, infrastructures specifications.
and buildings. It is based on a steel production in an
Electric Arc Furnace with 100% renewable electricity Application
supply with Guarantee of Origins. Steel sheet pile walls resist high pressure and can
support the massive height of soil with a small quantity
EcoSheetPile™ Plus are produced at the ArcelorMittal of steel compared to the applied loads. Steel sheet
sites Differdange and Esch-Belval in Luxembourg from piles are used worldwide in many kinds of permanent
ca. 100% scrap in an electric arc furnace route and are and temporary structures: quay walls and breakwaters
100% reusable and recyclable. The types of in harbours, locks, bank reinforcement on rivers and
EcoSheetPile™ Plus available are: Z-shaped, U- canals, pumping stations, bridge abutments, retaining
shaped, straight-web, and H-shaped. walls for underpasses, tunnels and underground car
parks, impervious containment walls, temporary
2 Environmental Product Declaration ArcelorMittal – EcoSheetPile™ Plus
cofferdams in land and in water, containment barriers,  Canadian standard association (CSA) CSA
and load bearing foundations, among others. 260W, CSA 300W, CSA 350W.
Technical Data
This EPD is valid for EcoSheetPile™ Plus steel sheet
piles of varied grades and geometries, as well as Base materials/Ancillary materials
different forms of delivery. The base material of EcoSheetPile™ Plus is iron.
Alloying elements are added in the form of ferroalloys
Constructional data or metals (the most common elements are Manganese
and Silicon). Steel sheet pile products according to EN
Name Value Unit
Density 7850 kg/m3 10248 are non-alloy steel products.Some small
quantities of other elements may be present in the
Modulus of elasticity 210000 N/mm2
steel (e.g. copper or nitrogen). The chemical
Coefficient of thermal expansion 12 10-6K-1
composition of the sheet piles depends mainly on the
Thermal conductivity 48 W/(mK)
steel grade.
Melting point 1536 °C
Shear modulus 81000 N/mm²
No substances listed on the “Candidate List of
Substances of Very High Concern for Authorisation” by
the European Chemicals Agency EC 1907-2006 are
Performance data of the product with respect to its
contained in the steel in declarable quantities.
characteristics in accordance with the relevant
technical provision (no CE-marking).
This product contains substances listed in the
candidate list (date: 22.2.2021) exceeding 0.1
Specific information on dimension tolerances,
percentage by mass: no
constructional data, as well as mechanical and
chemical properties can be found in the relevant
Reference service life
standards:
A reference service life for EcoSheetPile™ Plus is not
 European standards EN 10248‑1,
declared. These are construction products with many
EN 10248‑2. different applications purposes. The lifetime therefore
 ASTM international standards ASTM A572, will be limited by the service life of the work.
ASTM A6.
LCA: Calculation rules
Declared Unit production residues, and consideration of
The declaration refers to the functional unit of 1 metric related emissions
ton of EcoSheetPile™ Plus as specified in Part B
 Recycling of production/manufacturing scrap.
requirements on the EPD for structural steels.
Steel scrap is assumed to reach the end-of-
waste status once is shredded and sorted,
The background data are taken from GaBi ts
Documentation. thus becomes an input to the product system
in the inventory.
The final results reflect the weighted average per
production volume oft he two rolling lines in
Module C3 takes into account the sorting and
Differdange & Esch-Belval.
shredding of after-use steel that is recycled, as well as
the non-recovered scrap due to sorting efficiency
Declared unit
which is landfilled. A conservative value of 1% landfill
Name Value Unit
is considered.
Declared unit 1 t
Density 7850 kg/m3
Module C4 takes into account the waste disposal
Conversion factor to 1 kg 0.001 -
including physical pre-treatment and management of
the disposal site. Steel is an inert material which does
not require any specific treatment on disposal site.
System boundary
Module D refers to the end of life of the steel sheet
Type of the EPD: cradle-to-gate - with options. Module
piles, including reuse and recycling. In module D the
A1-A3, Module C3, Module C4 and Module D were
recycled material gets a credit in accordance with the
considered.
“value of scrap” methodology by WorldSteel and the
reused material receives a credit as avoided
Modules A1-A3 of the structural steel production
manufacturing of steel sheet piles.
include the following:
 The provision of resources, additives, and Comparability
energy Basically, a comparison or an evaluation of EPD data
 Transport of resources and additives to the is only possible if all the data sets to be compared
production site were created according to EN 15804 and the building
context, respectively the product-specific
 Production processes on-site including
characteristics of performance, are taken into account.
energy, production of additives, disposal of
3 Environmental Product Declaration ArcelorMittal – EcoSheetPile™ Plus
GaBi ts Software version 10.0.1.92 was used with GaBi Database 2021.2 to calculate this EPD.
LCA: Scenarios and additional technical information
The end of life for steel sheet piles consists of 85%
being retrieved for recycling or reuse and 15% landfill,
with the corresponding benefits and burdens. This is
based on the European Commission – Science
Research Development Report and internal
estimations.
Reuse
Part of the production is used for temporary works
(lasting up to 3 years). Steel sheet piles can be reused
up to 10 times without loss of their properties. The
frequency of reuse varies depending on the use case.
For instance, the same steel sheet piles can be used
successively for different parts of a construction site or
stocked by a company between two usages. According
to internal documentation within ArcelorMittal, currently
part of the sheet piles are reused several times,
leading to an overall reuse rate of 25%.
Recycling
Steel can be recycled to the same (or higher/lower)
quality of steel depending upon the metallurgy and
processing of the recycling route. Steel sheet piles can
be recycled without any problem after dismantling, and
recycling routes are well established. 85% of the sheet
piles are recovered for reuse and recycling. Since 25%
of the sheet piles are reused, the remaining 60% is
considered as recycled with the corresponding benefits
and burdens. In module D the recycled material gets a
credit or a burden based on the “value of scrap”
methodology by Worldsteel and the reused material
receives a credit as avoided manufacturing of
EcoSheetPile™ Plus.
For specific case studies, dedicated scenarios can be
calculated by contacting ArcelorMittal or using the data
provided in this document.
End of life (C1 - C4)
Name Value Unit
Reuse 250 kg
Recycling 600 kg
Landfilling 150 kg
Reuse, recovery and/or recycling potentials (D),
relevant scenario information
Name Value Unit
Reuse 25 %
Recycling 60 %
4 Environmental Product Declaration ArcelorMittal – EcoSheetPile™ Plus
LCA: Results
DESCRIPTION OF THE SYSTEM BOUNDARY (X = INCLUDED IN LCA; MND = MODULE NOT DECLARED;
MNR = MODULE NOT RELEVANT)
BENEFITS AND
CONSTRUCTI LOADS
PRODUCT STAGE ON PROCESS USE STAGE END OF LIFE STAGE BEYOND THE
STAGE SYSTEM
BOUNDARIES
5 Environmental Product Declaration ArcelorMittal – EcoSheetPile™ Plus
lairetam
waR
ylppus tropsnarT
gnirutcafunaM
eht
morf
tropsnarT
etis
eht
ot
etag
ylbmessA esU
ecnanetniaM
riapeR
tnemecalpeR tnemhsibrufeR
ygrene
lanoitarepO esu
retaw
lanoitarepO esu
noitcurtsnoc-eD
noitilomed tropsnarT
gnissecorp
etsaW
lasopsiD -esueR -yrevoceR -gnilcyceR laitnetop
A1 A2 A3 A4 A5 B1 B2 B3 B4 B5 B6 B7 C1 C2 C3 C4 D
X X X MND MND MND MND MNR MNR MNR MND MND MND MND X X X
RESULTS OF THE LCA - ENVIRONMENTAL IMPACT according to EN 15804+A1: 1 metric ton of
EcoSheetPile™ Plus
Parameter Unit A1-A3 C3 C4 D
Global warming potential [kg CO2-Eq.] 3.70E+2 1.60E+0 2.15E+0 3.24E+2
Depletion potential of the stratospheric ozone layer [kg CFC11-Eq.] 5.59E-11 4.69E-14 1.17E-14 -1.30E-11
Acidification potential of land and water [kg SO2-Eq.] 9.50E-1 2.99E-3 1.29E-2 4.34E-1
Eutrophication potential [kg (PO4)3--Eq.] 7.83E-2 4.48E-4 1.46E-3 1.50E-2
Formation potential of tropospheric ozone photochemical
[kg ethene-Eq.] 1.15E-1 2.60E-4 9.87E-4 1.80E-1
oxidants
Abiotic depletion potential for non-fossil resources [kg Sb-Eq.] 4.86E-4 4.70E-7 2.16E-7 8.05E-4
Abiotic depletion potential for fossil resources [MJ] 4.25E+3 1.82E+1 2.92E+1 2.86E+3
RESULTS OF THE LCA - INDICATORS TO DESCRIBE RESOURCE USE according to EN 15804+A1: 1
metric ton of EcoSheetPile™ Plus
Parameter Unit A1-A3 C3 C4 D
Renewable primary energy as energy carrier [MJ] 7.71E+3 1.22E+1 4.05E+0 -2.28E+3
Renewable primary energy resources as material utilization [MJ] 0.00E+0 0.00E+0 0.00E+0 0.00E+0
Total use of renewable primary energy resources [MJ] 7.71E+3 1.22E+1 4.05E+0 -2.28E+3
Non-renewable primary energy as energy carrier [MJ] 4.41E+3 2.82E+1 3.01E+1 2.70E+3
Non-renewable primary energy as material utilization [MJ] 0.00E+0 0.00E+0 0.00E+0 0.00E+0
Total use of non-renewable primary energy resources [MJ] 4.41E+3 2.82E+1 3.01E+1 2.70E+3
Use of secondary material [kg] 1.14E+3 0.00E+0 0.00E+0 0.00E+0
Use of renewable secondary fuels [MJ] 0.00E+0 0.00E+0 0.00E+0 0.00E+0
Use of non-renewable secondary fuels [MJ] 0.00E+0 0.00E+0 0.00E+0 0.00E+0
Use of net fresh water [m³] 1.37E+0 1.18E-2 7.43E-3 1.58E+0
RESULTS OF THE LCA – WASTE CATEGORIES AND OUTPUT FLOWS according to EN 15804+A1:
1 metric ton of EcoSheetPile™ Plus
Parameter Unit A1-A3 C3 C4 D
Hazardous waste disposed [kg] 1.81E-6 7.00E-9 3.20E-9 -1.52E-6
Non-hazardous waste disposed [kg] 4.97E+0 1.89E-2 1.50E+2 -4.70E+1
Radioactive waste disposed [kg] 5.17E-2 3.89E-3 3.15E-4 -1.31E-2
Components for re-use [kg] 0.00E+0 2.50E+2 0.00E+0 0.00E+0
Materials for recycling [kg] 0.00E+0 6.00E+2 0.00E+0 0.00E+0
Materials for energy recovery [kg] 0.00E+0 0.00E+0 0.00E+0 0.00E+0
Exported electrical energy [MJ] 0.00E+0 0.00E+0 0.00E+0 0.00E+0
Exported thermal energy [MJ] 0.00E+0 0.00E+0 0.00E+0 0.00E+0
References
EN 15804 PCR Part A
EN 15804+A1:2013, Sustainability of construction PCR - Part A: Calculation Rules for the Life Cycle
works — Environmental Product Declarations — Core Assessment and Requirements on the Project Report,
rules for the product category of construction products Institut Bauen und Umwelt e.V., 2021.
IBU 2021 PCR Part B
Institut Bauen und Umwelt e.V.: General Instructions Requirements on the EPD for Structural steels - Institut
for the EPD programme of Institut Bauen und Umwelt Bauen und Umwelt e.V., Berlin (pub.): From the range
e.V. Version 2.0, Berlin: Institut Bauen und Umwelt of Environmental Product
e.V., 2021. www.ibu-epd.com Declarations of Institute Construction and Environment
e.V. (IBU), 2017
GaBi ts Software ASTM A6
GaBi ts Software and Databases for Life Cycle ASTM A6 / A6M-19:2019, Standard Specification for
Engineering. LBP, University of Stuttgart und PE General Requirements for Rolled Structural Steel Bars,
International, 2013. Plates, Shapes, and Sheet Piling, ASTM International,
West Conshohocken, PA, 2019.
GaBi ts Documentation
GaBi ts Documentation of the GaBi datasets for Life CSA 260W, CSA 300W, CSA 350W
Cycle Engineering. LBP, Universitity of Stuttgart and CSA G40.20:2013, General requirements for rolled or
PE International, 2011. welded structural quality steel. Canadian Standard
http://gabi.sphera.com/support/gabi Association.
CSA G40.21:2013, General requirements for structural
EN 10248-1 quality steel. Canadian Standard Association.
EN 10248-1:1995, Hot rolled sheet piling of non alloy
steels - Part 1: Technical delivery conditions. CEN, Candidate List of Substances of Very High
1995. Concern for Authorization
Regulation (EC) No 1907/2006 of the European
EN 10248-2 Parliament and of the Council on the Registration,
EN 10248-2:1995, Hot rolled sheet piling of non alloy Evaluation, Authorisation and Restriction of Chemicals
steels - Part 2: Tolerances on shape and dimensions. (REACH)
CEN, 1995. https://echa.europa.eu/candidate-list-table
ASTM A572 European Commission – Science Research
ASTM A572 / A572M-21e1:2021, Standard Development Report
Specification for High-Strength Low-Alloy Columbium- Life-Cycle Assessment (LCA) for steel construction.
Vanadium Structural Steel, ASTM International, West Technical steel research. 2002
Conshohocken, PA, 2021.
6 Environmental Product Declaration ArcelorMittal – EcoSheetPile™ Plus
Publisher
Institut Bauen und Umwelt e.V. Tel +49 (0)30 3087748- 0
Panoramastr. 1 Fax +49 (0)30 3087748- 29
10178 Berlin Mail info@ibu-epd.com
Germany Web www.ibu-epd.com
Programme holder
Institut Bauen und Umwelt e.V. Tel +49 (0)30 - 3087748- 0
Panoramastr 1 Fax +49 (0)30 – 3087748 - 29
10178 Berlin Mail info@ibu-epd.com
Germany Web www.ibu-epd.com
Author of the Life Cycle
Assessment Tel +352 5313 3105
ArcelorMittal Commercial RPS – Fax -
Sheet piling Mail sheetpiling@arcelormittal.com
Rue de Luxembourg 66 Web sheetpiling.arcelormittal.com
4221 Esch-sur-Alzette
Luxembourg
Owner of the Declaration
ArcelorMittal Commercial RPS – Tel +352 5313 3105
Sheet piling Fax -
Rue de Luxembourg 66 Mail sheetpiling@arcelormittal.com
4221 Esch-sur-Alzette Web sheetpiling.arcelormittal.com
Luxembourg
