Environmental product declaration
in accordance with ISO 14025 and EN 15804+A2
EFG Lockable Storage special 240x40x1640+100mm
Owner of the declaration: Program operator:
EFG European Furniture Group AB The Norwegian EPD Foundation
Declaration number:
EFG Lockable Storage special 240x40x1640+100mm
Registration number:
Declared unit:
1 kg Issue date:
This declaration is based on Product Category Rules: Valid to:
CEN Standard EN 15804:2012+A1:2013 serves as core
EPD software:
PCR
The Norwegian EPD Foundation LCAno EPD generator ID: 365928
NPCR 026:2022 Part B for Furniture
1 / 11
General information
Product Owner of the declaration:
EFG Lockable Storage special 240x40x1640+100mm EFG European Furniture Group AB
Contact person: Christer Johansson
Phone:
e-mail: christer.johansson@efg.se
Program operator: Manufacturer:
The Norwegian EPD Foundation EFG European Furniture Group AB
Post Box 5250 Majorstuen, 0303 Oslo, Norway
Phone: +47 977 22 020
web: www.epd-norge.no
Declaration number: Place of production:
EFG European Furniture Group AB
, Norway
This declaration is based on Product Category Rules: Management system:
CEN Standard EN 15804:2012+A1:2013 serves as core PCR ISO 14001
NPCR 026:2022 Part B for Furniture
Statement of liability: Organisation no:
The owner of the declaration shall be liable for the underlying
information and evidence. EPD Norway shall not be liable with respect
to manufacturer information, life cycle assessment data and
evidences.
Declared unit: Issue date:
1 kg EFG Lockable Storage special 240x40x1640+100mm
Declared unit with option: Valid to:
A1,A2,A3,A4,A5,B2,B3,B4,C1,C2,C3,C4,D
Year of study:
2024
Functional unit: Comparability:
Storage special 240x40x1640+100mm excl. locks EPDs from programmes other than the Norwegian EPD Foundation
may not be comparable​
General information on verification of EPD from EPD tools: Development and verification of EPD:
Independent verification of data, other environmental information The declaration is created using EPD tool lca.tools ver EPD2022.03,
and the declaration according to ISO 14025:2010, § 8.1.3 and § 8.1.4. developed by LCA.no. The EPD tool is integrated in the company's
Verification of each EPD is made according to EPD-Norway’s management system, and has been approved by EPD Norway.
guidelines for verification and approval requiring that tools are i)
integrated into the company's environmental management system, ii) Developer of EPD: Andreas Mattisson
the procedures for use of the EPD tool are approved by EPD-Norway,
Reviewer of company-specific input data and EPD: Christer Johansson
and iii) the process is reviewed annually by an independent third
party verifier. See Appendix G of EPD-Norway's General Programme
Instructions for further information on EPD tools
Verification of EPD tool: Approved:
Independent third party verification of the EPD tool, background data Sign
and test-EPD in accordance with EPDNorway's procedures and
guidelines for verification and approval of EPD tools.
Third party verifier:
Erik Svanes, Norsus AS
(no signature required)
2 / 11
Product
Product description:
Storage special 240x40x1640+100mm excl. locks
Product specification
Storage special 240x40x1640+100mm excl. locks
Materials kg %
Metal - Stainless steel 0,20 0,25
Plastic - Melamine 1,20 1,49
Wood - Chipboard 79,00 98,26
Total 80,40 100,00
Packaging kg %
Packaging - Cardboard 2,20 28,21
Packaging - Pallet 5,60 71,79
Total incl. packaging 88,20 100,00
Technical data:
Market:
Reference service life, product
Reference service life, building
LCA: Calculation rules
Declared unit:
1 kg EFG Lockable Storage special 240x40x1640+100mm
Cut-off criteria:
All major raw materials and all the essential energy is included. The production processes for raw materials and energy flows with very small
amounts (less than 1%) are not included. These cut-off criteria do not​ apply for hazardous materials and substances.
Allocation:
The allocation is made in accordance with the provisions of EN 15804. Effects of primary production of recycled materials is allocated to the main
product in which the material was used. The recycling process and transportation of the material is allocated to this analysis.
Data quality:
Specific data for the product composition are provided by the manufacturer. They represent the production of the declared product and were
collected for EPD development in the year of study. Background data is based on registered EPDs according to EN 15804, Ostfold Research
databases, ecoinvent and other LCA databases. The data quality of the raw materials in A1 is presented in the table below.
Materials Source Data quality Year
Metal - Stainless steel ecoinvent 3.6 Database 2019
Packaging - Cardboard ecoinvent 3.6 Database 2019
Packaging - Pallet ecoinvent 3.6 Database 2019
Plastic - Melamine ecoinvent 3.6 Database 2019
Wood - Chipboard ecoinvent 3.6 Database 2019
3 / 11
System boundaries (X=included, MND=module not declared, MNR=module not relevant)
Construction Beyond the system
Product stage Use stage End of life stage
installation stage boundaries
A1 A2 A3 A4 A5 B1 B2 B3 B4 B5 B6 B7 C1 C2 C3 C4 D
X X X X X MND X X X MND MND MND X X X X X
System boundary:
Additional technical information:
waR slairetam tropsnarT gnirutcafunaM tropsnarT ylbmessA esU ecnanetniaM riapeR tnemecalpeR tnemhsibrufeR lanoitarepO ygrene esu lanoitarepO esu retaw -eD noitcurtsnoc noitilomed tropsnarT etsaW gnissecorp lasopsiD -yrevoceR-esueR laitnetop-gnilcyceR
4 / 11
LCA: Scenarios and additional technical information
Transport from production place to user (A4)
Capacity utilisation Value
Transport from production place to user (A4) Distance (km) Fuel/Energy Consumption Unit
(incl. return) % (Liter/tonn)
Truck, 16-32 tonnes, EURO 5 (km) 36,7 % 300 0,044 l/tkm 13,20
Assembly (A5) Unit Value
Waste, packaging, corrugated board box, to
kg 2,20
average treatment (kg)
Waste, packaging, Pallet, EUR wooden pallet,
kg 5,60
single use, average treatment (kg)
Capacity utilisation Value
Transport to waste processing (C2) Distance (km) Fuel/Energy Consumption Unit
(incl. return) % (Liter/tonn)
Truck, 16-32 tonnes, EURO 5 (km) 36,7 % 85 0,044 l/tkm 3,74
Waste processing (C3) Unit Value
Waste treatment per kg Non-hazardous waste,
kg 1,20
incineration with fly ash extraction - C3 (kg)
Waste treatment per kg Scrap steel, incineration
kg 0,20
with fly ash extraction (kg)
Waste treatment per kg Wood, incineration with
kg 79,00
fly ash extraction (kg)
Waste, materials to recycling (kg) kg 0,07
Disposal (C4) Unit Value
Landfilling of ashes and residues from
kg 0,13
incineration of Scrap steel (kg)
Landfilling of ashes from incineration of Non-
hazardous waste, process per kg ashes and kg 0,28
residues - C4 (kg)
Landfilling of ashes from incineration of Wood,
kg 0,91
process per kg ashes and residues (kg)
Benefits and loads beyond the system
Unit Value
boundaries (D)
Substitution of electricity, in Norway (MJ) MJ 55,65
Substitution of primary steel with net scrap (kg) kg 0,05
Substitution of thermal energy, district heating, in
MJ 841,97
Norway (MJ)
5 / 11
LCA: Results
The LCA results are presented below for the declared unit defined on page 2 of the EPD document.
Environmental impact
Indicator Unit A1 A2 A3 A4 A5 B2
GWP-total kg CO2 -eq -1,11E+02 1,16E+01 1,36E+01 4,41E+00 1,24E+01 0
GWP-fossil kg CO2 -eq 4,77E+01 1,16E+01 2,95E-01 4,41E+00 1,86E-01 0
GWP-biogenic kg CO2 -eq -1,58E+02 4,12E-03 1,33E+01 1,80E-03 1,22E+01 0
GWP-luluc kg CO2 -eq 1,38E-01 5,11E-03 1,92E-02 1,54E-03 5,04E-05 0
ODP kg CFC11 -eq 6,68E-06 2,52E-06 1,45E-07 1,01E-06 3,16E-08 0
AP mol H+ -eq 3,35E-01 1,60E-01 1,92E-03 1,80E-02 1,38E-03 0
EP-FreshWater kg P -eq 2,18E-03 7,49E-05 2,00E-05 3,46E-05 2,10E-06 0
EP-Marine kg N -eq 6,29E-02 4,13E-02 3,27E-04 5,35E-03 5,76E-04 0
EP-Terrestial mol N -eq 9,54E-01 4,59E-01 4,31E-03 5,91E-02 6,17E-03 0
POCP kg NMVOC -eq 3,05E-01 1,23E-01 9,81E-04 1,81E-02 1,60E-03 0
ADP-minerals&metals1 kg Sb-eq 1,02E-03 2,33E-04 1,18E-05 1,19E-04 3,31E-06 0
ADP-fossil1 MJ 8,91E+02 1,65E+02 3,46E+01 6,65E+01 2,27E+00 0
WDP1 m3 3,18E+03 1,19E+02 3,51E+03 6,34E+01 3,36E+00 0
Indicator Unit B3 B4 C1 C2 C3 C4 D
GWP-total kg CO2 -eq 0 0 0 1,25E+00 1,37E+02 4,13E-02 -5,12E+00
GWP-fossil kg CO2 -eq 0 0 0 1,25E+00 3,78E+00 4,12E-02 -4,94E+00
GWP-biogenic kg CO2 -eq 0 0 0 5,10E-04 1,33E+02 2,23E-05 -1,01E-02
GWP-luluc kg CO2 -eq 0 0 0 4,37E-04 1,95E-04 6,99E-06 -1,68E-01
ODP kg CFC11 -eq 0 0 0 2,85E-07 9,93E-08 5,34E-09 -3,56E-01
AP mol H+ -eq 0 0 0 5,11E-03 1,28E-02 1,61E-04 -4,05E-02
EP-FreshWater kg P -eq 0 0 0 9,81E-06 1,81E-05 5,42E-07 -4,37E-04
EP-Marine kg N -eq 0 0 0 1,51E-03 6,08E-03 5,17E-05 -1,32E-02
EP-Terrestial mol N -eq 0 0 0 1,68E-02 6,45E-02 5,85E-04 -1,43E-01
POCP kg NMVOC -eq 0 0 0 5,13E-03 1,58E-02 1,63E-04 -3,95E-02
ADP-minerals&metals1 kg Sb-eq 0 0 0 3,38E-05 4,66E-06 2,83E-07 -4,96E-05
ADP-fossil1 MJ 0 0 0 1,88E+01 8,21E+00 4,38E-01 -7,03E+01
WDP1 m3 0 0 0 1,80E+01 1,06E+01 3,67E+00 -8,66E+02
GWP Global warming potential; ODP Depletion potential of the stratospheric ozone layer; POCP Formation potential of tropospheric photochemical oxidants; AP
Acidification potential of land and water; EP Eutrophication potential; ADPM Abiotic depletion potential for non fossil resources; ADPE Abiotic depletion​ potential for
fossil resources
"Reading example: 9,0 E-03 = 9,0*10-3 = 0,009"
*INA Indicator Not Assessed
1. The results of this environmental impact indicator shall be used with care as the uncertainties on these results are high or as there is limited experienced with the
indicator
3. Eutrophication aquatic freshwater shall be in kg P-eq., there is a typo in EN 15804:2012+A2:2019 regarding this unit. Eutrophication calculated as PO4-eq is presented
on page 11
Remarks to environmental impacts
6 / 11
Additional environmental impact indicators
Indicator Unit A1 A2 A3 A4 A5 B2
PM Disease incidence 1,00E-05 6,56E-07 1,38E-08 3,18E-07 1,73E-08 0
IRP2 kgBq U235 -eq 2,69E+00 7,19E-01 1,19E+00 2,91E-01 8,55E-03 0
ETP-fw1 CTUe 1,53E+03 1,13E+02 1,83E+01 4,90E+01 2,68E+00 0
HTP-c1 CTUh 2,83E-07 0,00E+00 5,25E-10 0,00E+00 2,44E-10 0
HTP-nc1 CTUh 8,06E-07 1,27E-07 1,26E-08 5,29E-08 1,16E-08 0
SQP1 dimensionless 6,42E+03 8,56E+01 1,53E+01 4,59E+01 1,33E+00 0
Indicator Unit B3 B4 C1 C2 C3 C4 D
PM Disease incidence 0 0 0 9,00E-08 1,32E-07 2,19E-09 -2,44E-06
IRP2 kgBq U235 -eq 0 0 0 8,24E-02 1,69E-02 2,00E-03 -4,46E-01
ETP-fw1 CTUe 0 0 0 1,39E+01 2,28E+01 6,85E-01 -3,83E+02
HTP-c1 CTUh 0 0 0 0,00E+00 3,00E-09 3,40E-11 -7,23E-09
HTP-nc1 CTUh 0 0 0 1,50E-08 1,41E-07 1,22E-09 -3,58E-07
SQP1 dimensionless 0 0 0 1,30E+01 1,24E+00 1,32E+00 -4,67E+02
PM = Particulate Matter emissions; IRP = Ionizing radiation – human health; ETP-fw = Eco toxicity – freshwater; HTP-c = Human toxicity – cancer effects; HTP-nc =
Human toxicity – non cancer effects; SQP = Potential Soil Quality Index (dimensionless)
"Reading example: 9,0 E-03 = 9,0*10-3 = 0,009"
*INA Indicator Not Assessed
1. The results of this environmental impact indicator shall be used with care as the uncertainties on these results are high or as there is limited experienced with the
indicator
2. This impact category deals mainly with the eventual impact of low dose ionizing radiation on human health of the nuclear fuel cycle. It does not consider effects due
to possible nuclear accidents, occupational exposure nor due to radioactive waste disposal in underground facilities. Potential ionizing radiation from the soil, from
radon and from some construction materials is also not measured by this indicator.
7 / 11
Resource use
Indicator Unit A1 A2 A3 A4 A5 B2
PERE MJ 4,32E+02 1,94E+00 1,66E+01 9,39E-01 4,46E-02 0
PERM MJ 8,73E+02 0,00E+00 -7,03E+01 0,00E+00 -9,58E+01 0
PERT MJ 1,30E+03 1,94E+00 -5,37E+01 9,39E-01 -9,57E+01 0
PENRE MJ 8,91E+02 1,65E+02 3,47E+01 6,65E+01 2,27E+00 0
PENRM MJ 0,00E+00 0,00E+00 0,00E+00 0,00E+00 0,00E+00 0
PENRT MJ 8,91E+02 1,65E+02 3,47E+01 6,65E+01 2,27E+00 0
SM kg 9,94E-01 0,00E+00 0,00E+00 0,00E+00 0,00E+00 0
RSF MJ 2,47E+00 6,61E-02 6,44E-02 3,36E-02 1,33E-03 0
NRSF MJ 4,99E-02 2,07E-01 2,04E-01 1,20E-01 1,32E-02 0
FW m3 1,40E+00 1,45E-02 3,78E-02 7,00E-03 1,52E-03 0
Indicator Unit B3 B4 C1 C2 C3 C4 D
PERE MJ 0 0 0 2,66E-01 3,02E-01 2,14E-02 -4,31E+02
PERM MJ 0 0 0 0,00E+00 -7,03E+02 0,00E+00 0,00E+00
PERT MJ 0 0 0 2,66E-01 -7,03E+02 2,14E-02 -4,31E+02
PENRE MJ 0 0 0 1,88E+01 8,33E+00 4,38E-01 -7,03E+01
PENRM MJ 0 0 0 0,00E+00 0,00E+00 0,00E+00 0,00E+00
PENRT MJ 0 0 0 1,88E+01 8,33E+00 4,38E-01 -7,03E+01
SM kg 0 0 0 0,00E+00 0,00E+00 0,00E+00 0,00E+00
RSF MJ 0 0 0 9,52E-03 7,12E-03 5,35E-04 -7,34E-02
NRSF MJ 0 0 0 3,40E-02 0,00E+00 2,81E-01 -2,55E+01
FW m3 0 0 0 1,98E-03 1,69E-02 4,01E-04 -5,19E-01
RPEE Renewable primary energy resources used as energy carrier; RPEM Renewable primary energy resources used as raw materials; TPE Total use of renewable primary
energy; NRPE Non renewable primary energy resources used as energy carrier; NRPM Non renewable primary energy resources used as​ materials; TRPE Total use of non
renewable primary energy; SM Use of secondary materials; RSF Use of renewable secondary fuels; NRSF Use of non renewable secondary fuels; W Use of net fresh water
"Reading example: 9,0 E-03 = 9,0*10-3 = 0,009"
*INA Indicator Not Assessed
8 / 11
End of life - Waste
Indicator Unit A1 A2 A3 A4 A5 B2
HWD kg 2,24E-01 7,90E-03 1,81E-03 3,39E-03 0,00E+00 0
NHWD kg 7,93E+00 5,60E+00 1,14E-01 3,18E+00 7,80E+00 0
RWD kg 2,83E-03 1,13E-03 5,21E-04 4,53E-04 0,00E+00 0
Indicator Unit B3 B4 C1 C2 C3 C4 D
HWD kg 0 0 0 9,61E-04 0,00E+00 1,04E+00 -3,58E-03
NHWD kg 0 0 0 9,01E-01 1,20E+00 2,90E-01 -1,67E+00
RWD kg 0 0 0 1,28E-04 0,00E+00 2,57E-06 -3,65E-04
HW Hazardous waste disposed; NHW Non hazardous waste disposed; RW Radioactive waste disposed
"Reading example: 9,0 E-03 = 9,0*10-3 = 0,009"
*INA Indicator Not Assessed
End of life - Output flow
Indicator Unit A1 A2 A3 A4 A5 B2
CRU kg 0,00E+00 0,00E+00 0,00E+00 0,00E+00 0,00E+00 0
MFR kg 0,00E+00 0,00E+00 0,00E+00 0,00E+00 2,05E+00 0
MER kg 0,00E+00 0,00E+00 0,00E+00 0,00E+00 5,71E+00 0
EEE MJ 0,00E+00 0,00E+00 0,00E+00 0,00E+00 3,99E+00 0
EET MJ 0,00E+00 0,00E+00 0,00E+00 0,00E+00 6,04E+01 0
Indicator Unit B3 B4 C1 C2 C3 C4 D
CRU kg 0 0 0 0,00E+00 0,00E+00 0,00E+00 0,00E+00
MFR kg 0 0 0 0,00E+00 6,79E-02 0,00E+00 0,00E+00
MER kg 0 0 0 0,00E+00 8,04E+01 0,00E+00 0,00E+00
EEE MJ 0 0 0 0,00E+00 5,49E+01 0,00E+00 0,00E+00
EET MJ 0 0 0 0,00E+00 8,31E+02 0,00E+00 0,00E+00
CR Components for reuse; MR Materials for recycling; MER Materials for energy recovery; EEE Exported electric energy; ETE Exported thermal energy
"Reading example: 9,0 E-03 = 9,0*10-3 = 0,009"
*INA Indicator Not Assessed
Biogenic Carbon Content
Indicator Unit At the factory gate
Biogenic carbon content in product​ kg C 3,99E+01
Biogenic carbon content in accompanying packaging kg C 3,54E+00
Note: 1 kg biogenic carbon is equivalent to 44/12 kg CO2
9 / 11
Additional requirements
Greenhouse gas emissions from the use of electricity in the manufacturing phase
National production mix from import, low voltage (production of transmission lines, in addition to direct emissions and losses in grid) of applied
electricity for the manufacturing process (A3).
Electricity mix Source Amount Unit
Electricity, Sweden (kWh) ecoinvent 3.6 54,94 g CO2-eq/kWh
Dangerous substances
The product contains no substances given by the REACH Candidate list or the Norwegian priority list.
Indoor environment
Additional Environmental Information
Additional environmental impact indicators required in NPCR Part A for construction products
Indicator Unit A1 A2 A3 A4 A5 B2
GWPIOBC kg CO2 -eq 4,86E+01 1,16E+01 3,20E-01 4,41E+00 1,86E-01 0
Indicator Unit B3 B4 C1 C2 C3 C4 D
GWPIOBC kg CO2 -eq 0 0 0 1,25E+00 2,49E+00 4,51E-02 -5,07E+00
GWP-IOBC: Global warming potential calculated according to the principle of instantaneous oxidation. In order to increase the transparency of biogenic carbon​
contribution to climate impact, the indicator GWP-IOBC is required as it declares climate impacts calculated according to the principle of instantaneous oxidation.​
GWP-IOBC is also referred to as GWP-GHG in context to Swedish public procurement legislation.
10 / 11
Bibliography
ISO 14025:2010 Environmental labels and declarations - Type III environmental declarations - Principles and procedures.​
ISO 14044:2006 Environmental management - Life cycle assessment - Requirements and guidelines.​
EN 15804:2012+A1:2013 Environmental product declaration - Core rules for the product category of construction products.​
ISO 21930:2017 Sustainability in buildings and civil engineering works - Core rules for environmental product declarations of construction
products.​
ecoinvent v3, Allocation, cut-off by classification, Swiss Centre of Life Cycle Inventories.​
Iversen et al., (2018) eEPD v3.0 - Background information for EPD generator system. LCA.no report number 04.18​
Vold et al., (2019) EPD generator for Norsk Industri, Background information for industry application and LCA data, LCA.no report number 06.19.​
NPCR Part A: Construction products and services. Ver. 1.0. April 2017, EPD-Norge.​
NPCR 026 Part B for Furniture. Ver. 2.0 October 2018, EPD-Norge.
Program operator and publisher Phone: +47 977 22 020
The Norwegian EPD Foundation e-mail: post@epd-norge.no
Post Box 5250 Majorstuen, 0303 Oslo, Norway web: www.epd-norge.no
Owner of the declaration: Phone:
EFG European Furniture Group AB e-mail: christer.johansson@efg.se
, web: https://www.efg.se
Author of the Life Cycle Assessment Phone: +47 916 50 916
LCA.no AS e-mail: post@lca.no
Dokka 6B, 1671 web: www.lca.no
Developer of EPD generator Phone: +47 916 50 916
LCA.no AS e-mail: post@lca.no
Dokka 6B,1671 Kråkerøy web: www.lca.no
ECO Platform web: www.eco-platform.org
ECO Portal web: ECO Portal
11 / 11
