Environmental product declaration
in accordance with ISO 14025 and EN 15804+A2
Enya recliner with tilt and stepless adjustment and with a built-in footrest
Owner of the declaration: Program operator:
Helland Møbler AS The Norwegian EPD Foundation
Product: Declaration number:
Enya recliner with tilt and stepless adjustment and with a
built-in footrest NEPD-8461-8120-EN
Declared unit: Registration number:
1 pcs
NEPD-8461-8120-EN
This declaration is based on Product Category Rules:
Issue date: 12.12.2024
CEN Standard EN 15804:2012+A2:2019 serves as core
The Norwegian EPD Foundation PCR Valid to: 12.12.2029
OUTDATED NPCR 026:2018 Part B for furniture
EPD software:
LCAno EPD generator ID: 711990
1 / 12
General information
Product Owner of the declaration:
Enya recliner with tilt and stepless adjustment and with a built-in Helland Møbler AS
footrest Contact person: Joakim Helland
Phone: +47 958 09 013
e-mail: joakim.helland@helland.no
Program operator: Manufacturer:
The Norwegian EPD Foundation Helland Møbler AS
Post Box 5250 Majorstuen, 0303 Oslo, Norway Postboks 10
Phone: +47 977 22 020 6259 Stordal, Norway
web: www.epd-norge.no
Declaration number: Place of production:
Helland Baltic ÖU
NEPD-8461-8120-EN
Hapvali, Nõmme küla, Haapsalu linn
EE-90439 Läänemaa, Estonia
This declaration is based on Product Category Rules: Management system:
CEN Standard EN 15804:2012+A2:2019 serves as core PCR ISO 14001:2015, sertifikat nr 901085
OUTDATED NPCR 026:2018 Part B for furniture
Statement of liability: Organisation no:
The owner of the declaration shall be liable for the underlying 943 511 128
information and evidence. EPD Norway shall not be liable with respect
to manufacturer information, life cycle assessment data and
evidences.​
Declared unit: Issue date:
1 pcs Enya recliner with tilt and stepless adjustment and with a built-
12.12.2024
in footrest
Declared unit (cradle to gate) with option: Valid to:
A1-A3,A4,A5,B2,B3,B4,C1,C2,C3,C4,D 12.12.2029
Year of study:
2023
Functional unit: Comparability:
Production of one chair provided and maintained for a period of 15 EPD of construction products may not be comparable if they not
years. comply with EN 15804 and seen in a building context.
General information on verification of EPD from EPD tools: Development and verification of EPD:
Independent verification of data, other environmental information The declaration is created using EPD tool lca.tools ver EPD2022.03,
and the declaration according to ISO 14025:2010, § 8.1.3 and § 8.1.4. developed by LCA.no. The EPD tool is integrated in the company's
Verification of each EPD is made according to EPD-Norway’s management system, and has been approved by EPD Norway.
guidelines for verification and approval requiring that tools are i)
integrated into the company's environmental management system, ii) Developer of EPD: Oddrun Aunet Innselset
the procedures for use of the EPD tool are approved by EPD-Norway,
Reviewer of company-specific input data and EPD: Pawel Sosinski
and iii) the process is reviewed annually by an independent third
party verifier. See Appendix G of EPD-Norway's General Programme
Instructions for further information on EPD tools
Verification of EPD tool: Approved:
Independent third party verification of the EPD tool, background data
and test-EPD in accordance with EPDNorway's procedures and
guidelines for verification and approval of EPD tools.
Third party verifier:
Elisabet Amat, GREENIZE projects
(no signature required)
2 / 12
Product
Product description:
The Enya electrically adjustable recliner with a built-in footrest is a modern healthcare furniture piece that combines function with design, perfect
for both home and healthcare settings. The backrest and footrest can be adjusted independently, allowing the chair to be tailored to the user's
needs. The chair blends clean lines with ergonomic comfort, making it ideal for both relaxation and healthcare purposes. Its soft, supportive
padding offers an optimal seating experience, while its high quality ensures long-lasting use. The Enya recliner enhances any room with its elegant
design and is equally suitable for private homes as well as healthcare environments.
Product specification
Swing-, tilt- and gliding function
• 5 step adjustable neck support
• Stepless seat angle adjustment lock
Recycled share in Recycled share in
Materials kg %
material (kg) material (%)
Plastic -
6,10 24,60 0,00 0,00
Polypropylene (PP)
Powder coating 0,40 1,61 0,00 0,00
Metal - Steel 15,59 62,86 3,12 20,00
Textile - Polyester 2,71 10,93 0,00 0,00
Total 24,80 100,00 3,12
Recycled share in Recycled share in
Packaging kg %
material (kg) material (%)
Packaging - Plastic 0,20 3,20 0,00 0,00
Recycled
6,05 96,80 6,05 100,00
cardboard
Total incl.
31,05 100,00 9,17
packaging
Technical data:
Width: 74cm,
Height: 107cm,
Depth: 83cm,
Sitting height: 46cm,
Armrest height: 62cm,
Seat depth: 44-49cm,
Weight: 25,0kg (without cardboard)
Market:
Europa and USA
Reference service life, product
15 years
Reference service life, building
LCA: Calculation rules
Declared unit:
1 pcs Enya recliner with tilt and stepless adjustment and with a built-in footrest
Cut-off criteria:
All major raw materials and all the essential energy is included. The production processes for raw materials and energy flows with very small
amounts (less than 1%) are not included. These cut-off criteria do not apply for hazardous materials and substances.
Allocation:
The allocation is made in accordance with the provisions of EN 15804. Incoming energy and water and waste production in-house is allocated
equally among all products through mass allocation. Effects of primary production of recycled materials is allocated to the main product in which
the material was used. The recycling process and transportation of the material is allocated to this analysis.
Data quality:
Specific data for the product composition are provided by the manufacturer. They represent the production of the declared product and were
collected for EPD development in the year of study. Background data is based on registered EPDs according to EN 15804, Ostfold Research
databases, ecoinvent and other LCA databases. The data quality of the raw materials in A1 is presented in the table below.​
3 / 12
Materials Source Data quality Year
Metal - Steel ecoinvent 3.6 Database 2019
Packaging - Plastic ecoinvent 3.6 Database 2019
Plastic - Polypropylene (PP) ecoinvent 3.6 Database 2019
Powder coating Ecoinvent 3.6 Database 2019
Recycled cardboard Modified ecoinvent 3.6 Database 2019
Textile - Polyester ecoinvent 3.6 Database 2019
4 / 12
System boundaries (X=included, MND=module not declared, MNR=module not relevant)
Construction Beyond the system
Product stage Use stage End of life stage
installation stage boundaries
A1 A2 A3 A4 A5 B1 B2 B3 B4 B5 B6 B7 C1 C2 C3 C4 D
X X X X X MND X X X MND MND MND X X X X X
System boundary:
Additional technical information:
Transportation to an average customer in Copenhagen is 1000 km (A4: average European lorry > 32 tonnes)​
The use stage (B1) is represented by a scenario and includes vacuum cleaning of textile once a month. The PCR does not​
provide detailed guidelines for what should be included in the use stage. In the end of life stage, the transport distance for​
waste to waste processing is 72 km (C1). The reuse, recovery and recycling stage is beyond the system boundaries (D). It is​
assumed that the solution is dismantled and the materials recycled or combusted according to general Norwegian treatment of​
industrial waste (see the table below). This calculation includes only CO2 emissions (GWP) in the C-modules. The transport​
distance to reuse, recovery or recycling varies for each material, but the average distance is 373 km. The vehicles used and​
associated data are described in detail in [5].
waR slairetam tropsnarT gnirutcafunaM tropsnarT ylbmessA e​sU ecnanetniaM riapeR tnemecalpeR tnemhsibrufeR lanoitarepO ygrene esu lanoitarepO esu retaw -eD noitcurtsnoc noitilomed tropsnarT etsaW gnissecorp lasopsiD -yrevoceR-esueR laitnetop-gnilcyceR
5 / 12
LCA: Scenarios and additional technical information
The following information describe the scenarios in the different modules of the EPD.
Transportation to an average customer in Copenhagen is 1000 km (A4: average European lorry > 32 tonnes)​
The use stage (B1) is represented by a scenario and includes vacuum cleaning of textile once a month. The PCR does not​
provide detailed guidelines for what should be included in the use stage. In the end of life stage, the transport distance for​
waste to waste processing is 72 km (C1). The reuse, recovery and recycling stage is beyond the system boundaries (D). It is​
assumed that the solution is dismantled and the materials recycled or combusted according to general Norwegian treatment of​
industrial waste (see the table below). This calculation includes only CO2 emissions (GWP) in the C-modules. The transport​
distance to reuse, recovery or recycling varies for each material, but the average distance is 373 km. The vehicles used and​
associated data are described in detail in [5].
Capacity utilisation Value
Transport from production place to user (A4) Distance (km) Fuel/Energy Consumption Unit
(incl. return) % (Liter/tonne)
Truck, 16-32 tonnes, EURO 6 (km) 36,7 % 1000 0,043 l/tkm 43,00
Truck, 7.5-16 tonnes, EURO 6 (kgkm) 35,4 % 300 0,056 l/tkm 16,80
Assembly (A5) Unit Value
Waste, packaging, cardboard, 100 % recycled, to
kg 1,51
average treatment (kg)
Assembly (A5) Unit Value
Waste, Packaging, Plastic film(LDPE), to avergae
kg 0,75
treatment-A5 (kg)
Waste, Packaging, Cardboard, 100% recyled, to
kg 5
average treatment (kg)
Waste, Packaging, Corrugated board box, 0&
kg 0,245
recycled, to average treatment (kg)
Maintenance (B2) Unit Value
Electricity, European average (kWh) kWh/DU 11,70
Water, tap water (m3) m3/DU 0,78
Capacity utilisation Value
Transport to waste processing (C2) Distance (km) Fuel/Energy Consumption Unit
(incl. return) % (Liter/tonne)
Truck, 16-32 tonnes, EURO 6 (km) 36,7 % 85 0,043 l/tkm 3,66
Waste processing (C3) Unit Value
Waste treatment per kg Non-hazardous waste,
kg 0,40
incineration with fly ash extraction - C3 (kg)
Waste treatment per kg Textile, incineration with
kg 2,71
fly ash extraction (kg)
Waste treatment per kg Polypropylene (PP),
kg 6,10
incineration with fly ash extraction - C3 (kg)
Waste, materials to recycling (kg) kg 5,29
Waste treatment per kg Scrap steel, incineration
kg 15,59
with fly ash extraction (kg)
Disposal (C4) Unit Value
Landfilling of ashes from incineration of Non-
hazardous waste, process per kg ashes and kg 0,09
residues - C4 (kg)
Landfilling of ashes from incineration of Textile,
kg 0,14
soiled, process per kg ashes and residues (kg)
Landfilling of ashes from incineration of
Polypropylene, PP, process per kg ashes and kg 0,18
residues - C4 (kg)
Landfilling of ashes and residues from
kg 10,30
incineration of Scrap steel (kg)
Benefits and loads beyond the system
Unit Value
boundaries (D)
Substitution of electricity, in Norway (MJ) MJ 12,62
Substitution of thermal energy, district heating, in
MJ 190,97
Norway (MJ)
Substitution of primary steel with net scrap (kg) kg 4,23
6 / 12
LCA: Results
The LCA results are presented below for the declared unit defined on page 2 of the EPD document.
Environmental impact
Indicator Unit A1-A3 A4 A5 B2 B3
GWP-total kg CO2 -eq 1,03E+02 7,07E+00 2,59E+00 5,28E+00 0
GWP-fossil kg CO2 -eq 1,11E+02 7,07E+00 2,44E-02 5,23E+00 0
GWP-biogenic kg CO2 -eq -8,63E+00 3,02E-03 2,56E+00 3,66E-02 0
GWP-luluc kg CO2 -eq 1,17E-01 2,67E-03 8,08E-06 1,20E-02 0
ODP kg CFC11 -eq 9,88E-06 1,59E-06 5,16E-09 4,44E-07 0
AP mol H+ -eq 6,04E-01 2,03E-02 1,16E-04 3,05E-02 0
EP-FreshWater kg P -eq 5,33E-03 5,88E-05 2,01E-07 5,51E-04 0
EP-Marine kg N -eq 1,10E-01 3,97E-03 3,83E-05 3,92E-03 0
EP-Terrestial mol N -eq 1,21E+00 4,44E-02 4,14E-04 4,82E-02 0
POCP kg NMVOC -eq 4,30E-01 1,70E-02 1,19E-04 1,24E-02 0
ADP-minerals&metals1 kg Sb-eq 3,54E-03 2,12E-04 5,95E-07 4,39E-05 0
ADP-fossil1 MJ 1,86E+03 1,06E+02 3,42E-01 1,07E+02 0
WDP1 m3 7,39E+03 1,10E+02 4,33E-01 1,62E+03 0
Indicator Unit B4 C1 C2 C3 C4 D
GWP-total kg CO2 -eq 0 0 4,31E-01 2,06E+01 1,21E-01 -5,81E+00
GWP-fossil kg CO2 -eq 0 0 4,31E-01 1,66E+01 1,21E-01 -5,76E+00
GWP-biogenic kg CO2 -eq 0 0 1,78E-04 3,97E+00 1,06E-04 -4,85E-03
GWP-luluc kg CO2 -eq 0 0 1,53E-04 6,16E-05 3,58E-05 -4,02E-02
ODP kg CFC11 -eq 0 0 9,77E-08 2,82E-08 3,64E-08 -8,07E-02
AP mol H+ -eq 0 0 1,24E-03 3,05E-03 8,38E-04 -3,23E-02
EP-FreshWater kg P -eq 0 0 3,44E-06 4,93E-06 1,23E-06 -3,85E-04
EP-Marine kg N -eq 0 0 2,45E-04 1,39E-03 2,98E-04 -7,77E-03
EP-Terrestial mol N -eq 0 0 2,74E-03 1,50E-02 3,30E-03 -8,12E-02
POCP kg NMVOC -eq 0 0 1,05E-03 3,76E-03 9,49E-04 -3,22E-02
ADP-minerals&metals1 kg Sb-eq 0 0 1,19E-05 1,45E-06 2,03E-06 -9,14E-05
ADP-fossil1 MJ 0 0 6,52E+00 2,22E+00 2,70E+00 -5,50E+01
WDP1 m3 0 0 6,30E+00 9,57E-01 5,73E+00 4,43E+01
GWP-total = Global Warming Potential total; GWP-fossil = Global Warming Potential fossil fuels; GWP-biogenic = Global Warming Potential biogenic; GWP-luluc =
Global Warming Potential land use and land use change; ODP = Depletion potential of the stratospheric ozone layer; AP = Acidification potential, Accumulated
Exceedance; EP-freshwater = Eutrophication potential, fraction of nutrients reaching freshwater end compartment: EP-marine = Eutrophication potential, fraction of
nutrients reaching marine end compartment; EP-terrestrial = Eutrophication potential, Accumulated Exceedance; POCP = Formation potential of tropospheric ozone;
ADP-minerals&metals = Abiotic depletion potential for non-fossil resources; ADP-fossil = Abiotic depletion for fossil resources potential; WDP = Water (user)
deprivation potential, deprivation-weighted water consumption
"Reading example: 9,0 E-03 = 9,0*10-3 = 0,009"
*INA Indicator Not Assessed
1. The results of this environmental impact indicator shall be used with care as the uncertainties on these results are high or as there is limited experienced with the
indicator
Remarks to environmental impacts
7 / 12
Additional environmental impact indicators
Indicator Unit A1-A3 A4 A5 B2 B3
PM Disease incidence 6,53E-06 4,22E-07 1,71E-09 8,90E-08 0
IRP2 kgBq U235 -eq 5,95E+00 4,65E-01 1,46E-03 9,28E-01 0
ETP-fw1 CTUe 3,74E+03 8,01E+01 4,56E-01 7,67E+01 0
HTP-c1 CTUh 3,80E-07 0,00E+00 1,40E-11 2,74E-09 0
HTP-nc1 CTUh 3,40E-06 9,00E-08 5,72E-10 8,55E-08 0
SQP1 dimensionless 6,40E+02 7,13E+01 2,29E-01 2,60E+01 0
Indicator Unit B4 C1 C2 C3 C4 D
PM Disease incidence 0 0 2,64E-08 4,13E-08 1,52E-08 -9,39E-07
IRP2 kgBq U235 -eq 0 0 2,85E-02 5,16E-03 1,08E-02 -8,44E-02
ETP-fw1 CTUe 0 0 4,83E+00 1,21E+01 1,66E+00 -3,46E+02
HTP-c1 CTUh 0 0 0,00E+00 1,26E-09 6,10E-11 -2,40E-08
HTP-nc1 CTUh 0 0 5,28E-09 2,31E-08 1,66E-09 4,04E-07
SQP1 dimensionless 0 0 4,56E+00 3,92E-01 5,89E+00 -1,09E+02
PM = Particulate Matter emissions; IRP = Ionizing radiation – human health; ETP-fw = Eco toxicity – freshwater; HTP-c = Human toxicity – cancer effects; HTP-nc =
Human toxicity – non cancer effects; SQP = Soil Quality (dimensionless)
"Reading example: 9,0 E-03 = 9,0*10-3 = 0,009"
*INA Indicator Not Assessed
1. The results of this environmental impact indicator shall be used with care as the uncertainties on these results are high or as there is limited experienced with the
indicator
2. This impact category deals mainly with the eventual impact of low dose ionizing radiation on human health of the nuclear fuel cycle. It does not consider effects due
to possible nuclear accidents, occupational exposure nor due to radioactive waste disposal in underground facilities. Potential ionizing radiation from the soil, from
radon and from some construction materials is also not measured by this indicator.
8 / 12
Resource use
Indicator Unit A1-A3 A4 A5 B2 B3
PERE MJ 2,50E+02 1,60E+00 5,63E-03 2,05E+01 0
PERM MJ 3,54E+01 0,00E+00 -8,83E+00 0,00E+00 0
PERT MJ 2,86E+02 1,60E+00 -8,83E+00 2,05E+01 0
PENRE MJ 1,59E+03 1,06E+02 3,42E-01 1,07E+02 0
PENRM MJ 2,73E+02 0,00E+00 0,00E+00 0,00E+00 0
PENRT MJ 1,86E+03 1,06E+02 3,42E-01 1,07E+02 0
SM kg 9,17E+00 0,00E+00 0,00E+00 0,00E+00 0
RSF MJ 2,71E+00 5,76E-02 1,87E-04 1,50E+00 0
NRSF MJ 9,46E-01 2,07E-01 7,69E-04 3,93E-01 0
FW m3 1,04E+00 1,17E-02 1,61E-04 8,71E-01 0
Indicator Unit B4 C1 C2 C3 C4 D
PERE MJ 0 0 9,33E-02 9,36E-02 5,21E-02 -1,01E+02
PERM MJ 0 0 0,00E+00 0,00E+00 0,00E+00 0,00E+00
PERT MJ 0 0 9,33E-02 9,36E-02 5,21E-02 -1,01E+02
PENRE MJ 0 0 6,52E+00 2,31E+00 2,70E+00 -5,50E+01
PENRM MJ 0 0 0,00E+00 -2,65E+02 0,00E+00 0,00E+00
PENRT MJ 0 0 6,52E+00 -2,63E+02 2,70E+00 -5,50E+01
SM kg 0 0 0,00E+00 0,00E+00 0,00E+00 0,00E+00
RSF MJ 0 0 3,34E-03 2,19E-03 1,37E-03 1,51E-01
NRSF MJ 0 0 1,19E-02 0,00E+00 8,04E-02 -9,02E-01
FW m3 0 0 6,97E-04 4,52E-03 2,44E-03 -1,28E-01
PERE = Use of renewable primary energy excluding renewable primary energy resources used as raw materials; PERM = Use of renewable primary energy resources used
as raw materials; PERT = Total use of renewable primary energy resources; PENRE = Use of non renewable primary energy excluding non-renewable primary energy
resources used as raw materials; PENRM = Use of non renewable primary energy resources used as raw materials; PENRT = Total use of non renewable primary energy
resources; SM = Use of secondary materials; RSF = Use of renewable secondary fuels; NRSF = Use of non-renewable secondary fuels; FW = Net use of fresh water
"Reading example: 9,0 E-03 = 9,0*10-3 = 0,009"
*INA Indicator Not Assessed
9 / 12
End of life - Waste
Indicator Unit A1-A3 A4 A5 B2 B3
HWD kg 8,28E-01 5,60E-03 0,00E+00 1,63E-02 0
NHWD kg 2,49E+01 4,90E+00 1,51E+00 4,02E-01 0
RWD kg 5,73E-03 7,23E-04 0,00E+00 7,59E-04 0
Indicator Unit B4 C1 C2 C3 C4 D
HWD kg 0 0 3,36E-04 0,00E+00 1,05E+01 -2,49E-02
NHWD kg 0 0 3,17E-01 4,00E-01 1,58E-01 -2,28E+00
RWD kg 0 0 4,44E-05 0,00E+00 1,67E-05 -7,00E-05
HWD = Hazardous waste disposed; NHWD = Non-hazardous waste disposed; RWD = Radioactive waste disposed
"Reading example: 9,0 E-03 = 9,0*10-3 = 0,009"
*INA Indicator Not Assessed
End of life - Output flow
Indicator Unit A1-A3 A4 A5 B2 B3
CRU kg 0,00E+00 0,00E+00 0,00E+00 0,00E+00 0
MFR kg 5,31E-02 0,00E+00 1,40E+00 0,00E+00 0
MER kg 6,02E-01 0,00E+00 2,06E-06 0,00E+00 0
EEE MJ 3,53E-01 0,00E+00 8,64E-02 0,00E+00 0
EET MJ 5,34E+00 0,00E+00 1,31E+00 0,00E+00 0
Indicator Unit B4 C1 C2 C3 C4 D
CRU kg 0 0 0,00E+00 0,00E+00 0,00E+00 0,00E+00
MFR kg 0 0 0,00E+00 5,29E+00 0,00E+00 0,00E+00
MER kg 0 0 0,00E+00 2,48E+01 0,00E+00 0,00E+00
EEE MJ 0 0 0,00E+00 1,22E+01 0,00E+00 0,00E+00
EET MJ 0 0 0,00E+00 1,85E+02 0,00E+00 0,00E+00
CRU = Components for re-use; MFR = Materials for recycling; MER = Materials for energy recovery; EEE = Exported energy electrical; EET = Exported energy thermal
"Reading example: 9,0 E-03 = 9,0*10-3 = 0,009"
*INA Indicator Not Assessed
Biogenic Carbon Content
Indicator Unit At the factory gate
Biogenic carbon content in product kg C 0,00E+00
Biogenic carbon content in accompanying packaging kg C 2,80E+00
Note: 1 kg biogenic carbon is equivalent to 44/12 kg CO2
10 / 12
Additional requirements
Greenhouse gas emissions from the use of electricity in the manufacturing phase
National production mix from import, low voltage (production of transmission lines, in addition to direct emissions and losses in grid) of applied
electricity for the manufacturing process (A3).
Electricity mix Source Amount Unit
Electricity, Estonia (kWh) ecoinvent 3.6 926,93 g CO2-eq/kWh
Dangerous substances
The product contains no substances given by the REACH Candidate list.
Indoor environment
Our Furniture not contain any substances that affects indoor climate.
Additional Environmental Information
Key Environmental Indicators
Key environmental indicators Unit A1-A3 A4 A1-C4 A1-D
GWPtotal kg CO2 -eq 102,90 7,07 138,95 133,14
Total energy consumption MJ 1844,77 108,34 2094,79 1938,06
Amount of recycled materials % 29,53
Additional environmental impact indicators required in NPCR Part A for construction products
Indicator Unit A1-A3 A4 A5 B2 B3
GWPIOBC kg CO2 -eq 1,16E+02 7,07E+00 2,44E-02 5,64E+00 0
Indicator Unit B4 C1 C2 C3 C4 D
GWPIOBC kg CO2 -eq 0 0 4,31E-01 2,06E+01 1,31E-01 -8,11E+00
GWP-IOBC: Global warming potential calculated according to the principle of instantaneous oxidation. In order to increase the transparency of biogenic carbon
contribution to climate impact, the indicator GWP-IOBC is required as it declares climate impacts calculated according to the principle of instantaneous oxidation.
GWP-IOBC is also referred to as GWP-GHG in context to Swedish public procurement legislation.
Variants and Options
Key environmental indicators (A1-A3) for variants of this EPD
Variants Weight (kg) GWPtotal (kg CO2 -eq) Total energy consumption (MJ) Amount of recycled materials (%)
Enya recliner with tilt and stepless adjustment 25,60 94,82 1612,90 24,73
Enya Footstool 4,80 29,46 517,04 25,00
11 / 12
Bibliography
ISO 14025:2010 Environmental labels and declarations - Type III environmental declarations - Principles and procedures.
ISO 14044:2006 Environmental management - Life cycle assessment - Requirements and guidelines.
EN 15804:2012+A2:2019 Environmental product declaration - Core rules for the product category of construction products.
ISO 21930:2017 Sustainability in buildings and civil engineering works - Core rules for environmental product declarations of construction
products.
ecoinvent v3, Allocation, cut-off by classification, Swiss Centre of Life Cycle Inventories.
Iversen et al., (2021) eEPD v2021.09 Background information for EPD generator tool system verification, LCA.no Report number: 07.21
Ruud et al., (2023) EPD generator for NPCR026 Part B for Furniture - Background information for EPD generator application and LCA data,
LCA.no report number 01.23
NPCR Part A: Construction products and services. Ver. 2.0. March 2021, EPD-Norge.
NPCR 026 Part B for Furniture. Ver. 2.0 March 2022, EPD-Norge.
Program operator and publisher Phone: +47 977 22 020
The Norwegian EPD Foundation e-mail: post@epd-norge.no
Post Box 5250 Majorstuen, 0303 Oslo, Norway web: www.epd-norge.no
Owner of the declaration: Phone: +47 958 09 013
Helland Møbler AS e-mail: joakim.helland@helland.no
Postboks 10, 6259 Stordal, Norway web: www.helland.no
Author of the Life Cycle Assessment Phone: +47 916 50 916
LCA.no AS e-mail: post@lca.no
Dokka 6A, 1671 Kråkerøy, Norway web: www.lca.no
Developer of EPD generator Phone: +47 916 50 916
LCA.no AS e-mail: post@lca.no
Dokka 6A, 1671 Kråkerøy, Norway web: www.lca.no
ECO Platform web: www.eco-platform.org
ECO Portal web: ECO Portal
12 / 12
