ENVIRONMENTAL PRODUCT DECLARATION
as per ISO 14025 and EN 15804+A2
Owner of the Declaration dormakaba International Holding GmbH
Publisher Institut Bauen und Umwelt e.V. (IBU)
Programme holder Institut Bauen und Umwelt e.V. (IBU)
Declaration number EPD-DOR-20230053-CBA1-EN
Issue date 30.06.2023
Valid to 29.06.2028
ES 200
dormakaba
www.ibu-epd.com | https://epd-online.com
General Information
dormakaba ES 200
Programme holder Owner of the declaration
IBU – Institut Bauen und Umwelt e.V. dormakaba International Holding GmbH
Hegelplatz 1 DORMA Platz 1
10117 Berlin 58256 Ennepetal
Germany Germany
Declaration number Declared product / declared unit
EPD-DOR-20230053-CBA1-EN 1 piece of the product: Automatic Sliding Door Operator ES 200, consisting
of the following items:
• ES 200 Standard Sliding Door Operator
• Product packaging
This declaration is based on the product category rules: Scope:
Drive systems for automatic doors and gates, 01.08.2021 This Environmental Product Declaration refers to a specific sliding door
(PCR checked and approved by the SVR) operator ES 200 Standard manufactured by dormakaba. This EPD is also
representative for the ES 200-2D, ES 200 EASY and ES 200 EASYplus.
The production site is located in Ennepetal (Germany). Green electricity is
Issue date being used at this production site.
30.06.2023
Data represents the year 2022.
The owner of the declaration shall be liable for the underlying information
and evidence; the IBU shall not be liable with respect to manufacturer
Valid to
information, life cycle assessment data and evidences.
29.06.2028
The EPD was created according to the specifications of EN 15804+A2. In
the following, the standard will be simplified as EN 15804.
Verification
The standard EN 15804 serves as the core PCR
Independent verification of the declaration and data according to ISO
14025:2011
internally X externally
Dipl.-Ing. Hans Peters
(Chairman of Institut Bauen und Umwelt e.V.)
Florian Pronold Dr.-Ing. Wolfram Trinius,
(Managing Director Institut Bauen und Umwelt e.V.) (Independent verifier)
1 Environmental-Product Declaration - dormakaba - ES 200
Product
Product description/Product definition Base materials/Ancillary materials
The automatic sliding door operator is a solution for any fields The major material composition including the packaging of the
of application and scope of operation. The ES 200 allows product is listed below:
dormakaba to supply a drive system that covers all applications Name Value Unit
due to its modular construction with a low number of
Aluminium 41 %
components. The modular and flexible drive system is available
Steel 26 %
in the following variants:
Electronics 14 %
• ES 200 Standard
Paper 12 %
• ES 200 2D
• ES 200 EASY Plastic 7 %
• ES 200 EASYplus.
For the use and application of the product the respective
The product includes partial articles which contain substances
national provisions at the place of use apply. For ES 200 the
listed in the Candidate List of REACH Regulation1907/2006/EC
standards which can be applied are the following:
(date: 17.01.2023) exceeding 0.1 percentage by mass: yes
• EN 18650
• EN 16005 • Lead (Pb): 7439-92-1 (CAS-No) is included in the
• EN 60335 battery and some of the alloys used. The concentration
• EN 61000 in each individual alloy does not exceed 4.0% (by
• ISO 13849 mass).
• Machinery Directive 2006/42/EC
• 2011/65/EU ROHS3 Directive The Candidate List can be found on the ECHA websiteaddress:
https:echa.europa.eu/de/home.
The CE marking takes into account the proof of conformity with
Reference service life
the respective harmonized standards based on the legal
provisions above. The reference service life for the ES 200 amounts to 10 years
and depends on the application and frequency of use. For
Application repairs and renewals, suitable spare parts are available. The
The automatic sliding door operator ES 200 is used as a drive sliding door operators are tested and certified EN 16005,
for automating sliding door systems as well as escape and meaning they are designed to withstand a minimum of
rescue routes. Applications are available for single- and double 1.000.000 cycles.
leaf doors.
Technical Data
The ES 200 has following technical properties:
Name Value Unit
Height maximum 150 mm
Installation depth 180 mm
Opening and closing force maximum 150 N
Opening speed maximum 70 cm/s
Closing speed maximum 50 cm/s
Hold open time maximum 180 s
Supply voltage, frequency maximum 60 Hz
Class of protection 20 IP
Performance data of the product with respect to its
characteristics in accordance with the relevant technical
provision which can be applied are mentioned above.
LCA: Calculation rules
Declared Unit Production - Module A1-A3
The declared unit is 1 piece of the product: ES 200 The product stage includes:
Name Value Unit — A1, raw material extraction, processing and mechanical
Declared unit 1 pce. treatments, processing of secondary material input (e.g.
recycling processes), — A2, transport to the manufacturer,
Mass of declared product 40,41 kg
— A3, manufacturing and assembly including provision of all
materials, products and energy, as well as waste processing up
System boundary
to the end-of waste state.
The type of EPD is: cradle to gate with options, modules C1–
C4, and module D (A1–A3 + C + D and additional modules: A4
+ A5 + B6)
2 Environmental-Product Declaration - dormakaba - ES 200
Construction stage - Modules A4-A5 Module D (Benefits and loads beyond the system boundary)
The construction process stage includes: includes:
— A4, transport to the building site; — D, recycling potentials, expressed as net impacts and
— A5, installation into the building; benefits.
including provision of all materials, products and energy, as well
as waste processing up to the end-of waste state or disposal of Geographic Representativeness
final residues during the construction process stage. Land or region, in which the declared product system is
manufactured, used or handled at the end of the product´s
Use stage - Module B6 lifespan: Germany
The use stage related to the operation of the building includes:
— B6, operational energy use
Comparability
Basically, a comparison or an evaluation of EPD data is only
End-of-life stage– Modules C1-C4 and D
possible if all the data sets to be compared were created
The end-of-life stage includes:
according to EN 15804 and the building context, respectively
— C1, de-construction, demolition:
the product-specific characteristics of performance, are taken
— C2, transport to waste processing;
into account. Background database: GaBi, SP40
— C3, waste processing for reuse, recovery and/or recycling;
— C4, disposal;
including provision and all transport, provision of all materials,
products and related energy and water use.
LCA: Scenarios and additional technical information
Characteristic product properties biogenic carbon
Information on describing the Biogenic Carbon Content at Operational energy use (B6)
factory gate
Name Value Unit
Name ValueUnit
Electricity consumption for 1 year 189.29 kWh
kg
Biogenic carbon content in product 0.276 Days per year in use 365 days
C
Active state (hours/day) 1.8 h
Biogenic carbon content in accompanying kg
1.569 Idle state (hours/day) 22.2 h
packaging C
Electrical power active state 14.31 W
Electrical power idle state 22.2 W
The following technical scenario information is required for the
declared modules End of life (C1-C4)
Transport to the building site (A4) C1: The product dismantling from the building is done manually
Name Value Unit without environmental burden.
Litres of fuel (per 1 kg) 0.00276 l/100km Name Value Unit
Capacity utilisation (including empty runs) 55 % Collected separately waste type 36.2 kg
Transport distance via medium truck 100 km Recycling 32.2 kg
Energy recovery 2.75 kg
The product is transported via truck and ship. The product is
stored in the dormakaba logistic center in Germany. The main Landfilling 1.17 kg
distribution region is Europe. Transport to waste management 50 km
In order to allow scaling to a specific point of installation 100 km
The product is disassembled in a recycling process.
are declared as well.
Material recycling is then assumed for the metals and
electronics. The plastic components are assumed to be
Installation into the building (A5) incinerated with energy recovery. Electromechanics and minor
Name Value Unit proportions of residues arising from the recycling process are
landfilled. Region for the End of Life is: Global.
Waste packaging (paper and plastic) 4,26 kg
Reuse, recovery and/or recycling potentials (D), relevant
Reference service life scenario information
The collection rate is 100%.
Name Value Unit
Life Span according to the manufacturer 10 a
3 Environmental-Product Declaration - dormakaba - ES 200
LCA: Results
DESCRIPTION OF THE SYSTEM BOUNDARY (X = INCLUDED IN LCA; ND = MODULE OR INDICATOR NOT DECLARED; MNR =
MODULE NOT RELEVANT)
Benefits and
Construction loads beyond
Product stage Use stage End of life stage
process stage the system
boundaries
la ire ta m w a Ry lp p u s tro p s n a rT g n iru tc a fu n a M e h t m o rf tro p s n a rTe tis e h t o t e ta g y lb m e s s A e s U e c n a n e tn ia M ria p e R tn e m e c a lp e R tn e m h s ib ru fe R y g re n e la n o ita re p Oe s u re ta w la n o ita re p Oe s u n o itc u rts n o c -e Dn o itilo m e d tro p s n a rT g n is s e c o rp e ts a W la s o p s iD -e s u e R-y re v o c e R-g n ilc y c e Rla itn e to p
A1 A2 A3 A4 A5 B1 B2 B3 B4 B5 B6 B7 C1 C2 C3 C4 D
X X X X X MND MND MNR MNR MNR X MND X X X X X
RESULTS OF THE LCA - ENVIRONMENTAL IMPACT according to EN 15804+A2: 1 piece ES 200
Parameter Unit A1-A3 A4 A5 B6 C1 C2 C3 C4 D
GWP-total kg CO 2 eq 2.17E+02 3.53E-01 6.04E+00 7.66E+02 0 1.57E-01 8.36E+00 6.4E-02 -1.19E+02
GWP-fossil kg CO 2 eq 2.24E+02 3.38E-01 1.51E-01 7.62E+02 0 1.5E-01 7.01E+00 6.3E-02 -1.18E+02
GWP-biogenic kg CO 2 eq -7.59E+00 1.6E-02 5.89E+00 2.54E+00 0 7E-03 1.34E+00 2.17E-04 -3.48E-01
GWP-luluc kg CO 2 eq 1.4E-01 8.04E-06 9.94E-05 1.1E+00 0 3.58E-06 4.08E-04 1.83E-04 -2E-02
ODP kg CFC11 eq 4.11E-09 3.57E-17 1.09E-15 1.68E-11 0 1.59E-17 3.69E-15 2.35E-16 -8.15E-10
AP mol H+ eq 1.01E+00 3.38E-04 2E-03 1.68E+00 0 1.51E-04 1E-03 4.55E-04 -4.59E-01
EP-freshwater kg P eq 4.13E-04 7.23E-08 2.13E-07 2E-03 0 3.22E-08 5.87E-07 1.09E-07 -6.35E-05
EP-marine kg N eq 1.44E-01 1.08E-04 6.11E-04 3.74E-01 0 4.79E-05 3.44E-04 1.17E-04 -5.8E-02
EP-terrestrial mol N eq 1.55E+00 1E-03 8E-03 3.93E+00 0 5.32E-04 7E-03 1E-03 -6.23E-01
kg NMVOC
POCP 4.51E-01 3.04E-04 2E-03 1.02E+00 0 1.35E-04 9.49E-04 3.55E-04 -1.89E-01
eq
ADPE kg Sb eq 6.4E-03 1.01E-08 1.72E-08 2.21E-04 0 4.51E-09 5.1E-08 5.7E-09 -3E-03
ADPF MJ 2.9E+03 4.79E+00 1.91E+00 1.34E+04 0 2.13E+00 3.53E+00 8.32E-01 -1.64E+03
m3 world eq
WDP 3.61E+01 6.62E-04 7.49E-01 1.66E+02 0 2.95E-04 8.56E-01 7E-03 -6.45E+00
deprived
GWP = Global warming potential; ODP = Depletion potential of the stratospheric ozone layer; AP = Acidification potential of land and water; EP =
Eutrophication potential; POCP = Formation potential of tropospheric ozone photochemical oxidants; ADPE = Abiotic depletion potential for non-fossil
resources; ADPF = Abiotic depletion potential for fossil resources; WDP = Water (user) deprivation potential)
RESULTS OF THE LCA - INDICATORS TO DESCRIBE RESOURCE USE according to EN 15804+A2: 1 piece ES 200
Parameter Unit A1-A3 A4 A5 B6 C1 C2 C3 C4 D
PERE MJ 1.06E+03 1.5E-02 5.15E+01 5.94E+03 0 7E-03 9.9E+00 1.09E-01 -7.04E+02
PERM MJ 6.01E+01 0 -5.11E+01 0 0 0 -9E+00 0 0
PERT MJ 1.12E+03 1.5E-02 3.47E-01 5.94E+03 0 7E-03 8.97E-01 1.09E-01 -7.04E+02
PENRE MJ 2.83E+03 4.8E+00 1.91E+00 1.34E+04 0 2.13E+00 7.69E+01 8.32E-01 -1.64E+03
PENRM MJ 7.34E+01 0 0 0 0 0 -7.34E+01 0 0
PENRT MJ 2.91E+03 4.8E+00 1.91E+00 1.34E+04 0 2.13E+00 3.53E+00 8.32E-01 -1.64E+03
SM kg 3.26E+00 0 0 0 0 0 0 0 0
RSF MJ 0 0 0 0 0 0 0 0 0
NRSF MJ 0 0 0 0 0 0 0 0 0
FW m3 2.5E+00 2.71E-05 1.8E-02 6.87E+00 0 1.21E-05 2E-02 2.1E-04 -1.27E+00
PERE = Use of renewable primary energy excluding renewable primary energy resources used as raw materials; PERM = Use of renewable primary
energy resources used as raw materials; PERT = Total use of renewable primary energy resources; PENRE = Use of non-renewable primary energy
excluding non-renewable primary energy resources used as raw materials; PENRM = Use of non-renewable primary energy resources used as raw
materials; PENRT = Total use of non-renewable primary energy resources; SM = Use of secondary material; RSF = Use of renewable secondary fuels;
NRSF = Use of non-renewable secondary fuels; FW = Use of net fresh water
RESULTS OF THE LCA – WASTE CATEGORIES AND OUTPUT FLOWS according to EN 15804+A2:
1 piece ES 200
Parameter Unit A1-A3 A4 A5 B6 C1 C2 C3 C4 D
HWD kg 3.01E-05 4.65E-10 2.81E-09 5.55E-06 0 2.07E-10 1.26E-08 1.27E-08 -1.53E-05
NHWD kg 4.41E+01 4.9E-04 1.89E-01 9.51E+00 0 2.18E-04 7.36E-01 4.18E+00 -2.64E+01
RWD kg 1.44E-01 5.15E-06 1E-04 2.03E+00 0 2.29E-06 1.37E-04 9.47E-06 -1.7E-01
CRU kg 0 0 0 0 0 0 0 0 0
MFR kg 0 0 0 0 0 0 2.83E+01 0 0
MER kg 0 0 0 0 0 0 0 0 0
EEE MJ 0 0 9.14E+00 0 0 0 1.5E+01 0 0
EET MJ 0 0 1.66E+01 0 0 0 3.34E+01 0 0
4 Environmental-Product Declaration - dormakaba - ES 200
HWD = Hazardous waste disposed; NHWD = Non-hazardous waste disposed; RWD = Radioactive waste disposed; CRU = Components for re-use;
MFR = Materials for recycling; MER = Materials for energy recovery; EEE = Exported electrical energy; EET = Exported thermal energy
RESULTS OF THE LCA – additional impact categories according to EN 15804+A2-optional:
1 piece ES 200
Parameter Unit A1-A3 A4 A5 B6 C1 C2 C3 C4 D
Disease
PM 1.05E-05 1.78E-09 9.37E-09 1.41E-05 0 7.91E-10 1.69E-08 5.63E-09 -6.96E-06
incidence
IR kBq U235 eq 2.71E+01 7.36E-04 1.6E-02 3.34E+02 0 3.27E-04 1.3E-02 9.75E-04 -3.4E+01
ETP-fw CTUe 1.06E+03 3.4E+00 9.05E-01 5.73E+03 0 1.51E+00 1.34E+00 4.75E-01 -5.7E+02
HTP-c CTUh 2.76E-07 6.39E-11 4.79E-11 1.58E-07 0 2.84E-11 1.14E-10 7.04E-11 -2.45E-08
HTP-nc CTUh 2.94E-06 2.73E-09 2.07E-09 5.83E-06 0 1.22E-09 1.1E-08 7.76E-09 -9.43E-07
SQP SQP 1.23E+03 1.2E-02 5.06E-01 4.27E+03 0 5E-03 1.05E+00 1.73E-01 -5.8E+01
PM = Potential incidence of disease due to PM emissions; IR = Potential Human exposure efficiency relative to U235; ETP-fw = Potential comparative
Toxic Unit for ecosystems; HTP-c = Potential comparative Toxic Unit for humans (cancerogenic); HTP-nc = Potential comparative Toxic Unit for humans
(not cancerogenic); SQP = Potential soil quality index
Disclaimer 1 – for the indicator 'Potential Human exposure efficiency relative to U235'. This impact category deals mainly with the
eventual impact of low-dose ionizing radiation on human health of the nuclear fuel cycle. It does not consider effects due to possible
nuclear
accidents, occupational exposure or radioactive waste disposal in underground facilities. Potential ionizing radiation from the soil,
radon and from some construction materials is also not measured by this indicator.
Disclaimer 2 – for the indicators 'abiotic depletion potential for non-fossil resources', 'abiotic depletion potential for fossil resources',
'water (user) deprivation potential, deprivation-weighted water consumption', 'potential comparative toxic unit for ecosystems', 'potential
comparative toxic unit for humans –
cancerogenic', 'Potential comparative toxic unit for humans - not cancerogenic', 'potential soil quality index'. The results of this
environmental impact indicator shall be used with care as the uncertainties on these results are high as there is limited experience with
the indicator.
This EPD was created using a software tool.
References
EN 18650 ROHS3 Directive
EN 186501: 2010, Powered pedestrian doors Part 1: Directive 2011/65/EU of the European Parliament and of the
Product requirements and test methods Council of 8 June 2011 on the restriction of the use of certain
hazardous substances in electrical and electronic equipment
EN 18650
EN 186502: 2010, Powered pedestrian doors Part 2: Further References
Safety at powered pedestrian doors
IBU 2021
EN 16005 General Instructions for the EPD programme of Institut Bauen
EN 16005: 2013-01, Power operated pedestrian doorsets und Umwelt e.V. Version 2.0, Berlin: Institut Bauen und Umwelt
Safety in use - Requirements and test methods e.V., 2021. www.ibu-epd.com
EN 60335 GaBi
EN 60335-1, -2-103:2020 08, Household and similar electrical Sphera Solutions GmbH Gabi Software System and Database
appliances - Safety - Part 1: General requirements for Life Cycle Engineering 1992-2020 Version 10.0.0.71
University of Stuttgart Leinfelden-Echterdingen
EN 61000
EN 61000 -1-2: 2017-07, Electromagnetic compatibility (EMC) - GaBi ts documentation
Part 1-2: General Methodology for the achievement of GaBi life cycle inventory data documentation
functional safety of electrical and electronic systems including (https://www.gabisoftware.
equipment with regard to electromagnetic phenomena com/support/gabi/gabidatabase- 2020-lci-documentation/).
ISO 13849 LCA-tool dormakaba
ISO 138491: 2021-08, Safety of machinery Safety-related parts LCA tool, ENS (drive system) LCA-Tool No.: IBU-DOR-202108-
of control systems - Part 1: LT1-EN Developed by Sphera Solutions GmbH.
General principles for design
PCR Part A
Machinery Directive PCR – Part A: Calculation Rules for the Life Cycle Assessment
Directive 2006/42/EC of the European Parliament and of the and Requirements on the Project Re-port according to EN
Council on machinery, and amending Directive 95/16/EC 15804+A2:2019, Version 1.0, Institut Bauen und Umwelt e.V.,
www.ibu-epd.com.
REACH
Regulation (EC) No 1907/2006 of the European Parliament and PCR Part B
of the Council on the Registration, Evaluation, Authorisation PCR – Part B: Requirements on the EPD for Building Hardware
and Restriction of Chemicals (REACH) product, version 1.2, Institut Bauen und Umwelt e.V., www.ibu-
epd.com, 2020.
5 Environmental-Product Declaration - dormakaba - ES 200
Publisher
Institut Bauen und Umwelt e.V. +49 (0)30 3087748- 0
Hegelplatz 1 info@ibu-epd.com
10117 Berlin www.ibu-epd.com
Germany
Programme holder
Institut Bauen und Umwelt e.V. +49 (0)30 3087748- 0
Hegelplatz 1 info@ibu-epd.com
10117 Berlin www.ibu-epd.com
Germany
Author of the Life Cycle Assessment
dormakaba International Holding GmbH +49 2333 793-0
DORMA Platz 1 info.de@dormakaba.com
58256 Ennepetal www.dormakaba.com
Germany
Owner of the Declaration
dormakaba International Holding GmbH +49 2333 793-0
DORMA Platz 1 info.de@dormakaba.com
58256 Ennepetal www.dormakaba.com
Germany
6 Environmental-Product Declaration - dormakaba - ES 200
