ENVIRONMENTAL PRODUCT DECLARATION
as per ISO 14025 and EN 15804+A2
Owner of the Declaration dormakaba International Holding GmbH
Publisher Institut Bauen und Umwelt e.V. (IBU)
Programme holder Institut Bauen und Umwelt e.V. (IBU)
Declaration number EPD-DOR-20210283-CBC1-EN
Issue date 25.02.2022
Valid to 24.02.2027
ES 400 System - Sliding Door Operator
Dormakaba
www.ibu-epd.com | https://epd-online.com
General Information
Dormakaba ES 400 System - Sliding Door Operator
Programme holder Owner of the declaration
IBU – Institut Bauen und Umwelt e.V. dormakaba International Holding GmbH
Hegelplatz 1 DORMA Platz 1
10117 Berlin 58256 Ennepetal
Germany Germany
Declaration number Declared product / declared unit
EPD­DOR­20210283­CBC1­EN 1 piece of the product: ES 400 System ­ sliding door operator, consisting of
the following items:
­ one (1) ES 420 drive unit kit double leaf
­ one (1) ES 400 slide rail complete 3m
­ two (2) ES 400 adapter unit heavy load single leaf
­ packaging
This declaration is based on the product category rules: Scope:
Drive systems for automatic doors and gates, 01.08.2021 This declaration refers to a specific product. This EPD refers to the entire
(PCR checked and approved by the SVR) lifecycle of a representative ES 420 drive system for double leaf doors.
This Environmental Product Declaration is also representative for the ES
410 door operator for single leaf doors. The production locations are
Issue date located in Zusmarshausen and Ennepetal, Germany. Green electricity is
used at the production facilities.
25.02.2022
The material and energy flows were taken into consideration accordingly.
The year of data collection is 2021.
Valid to
The owner of the declaration shall be liable for the underlying information
24.02.2027 and evidence; the IBU shall not be liable with respect to manufacturer
information, life cycle assessment data and evidences.
The EPD was created according to the specifications of EN 15804+A2. In
the following, the standard will be simplified as EN 15804.
Verification
The standard EN 15804 serves as the core PCR
Independent verification of the declaration and data according to ISO
14025:2011
internally X externally
Dipl.­Ing. Hans Peters
(Chairman of Institut Bauen und Umwelt e.V.)
Florian Pronold Dr.­Ing. Wolfram Trinius,
(Managing Director Institut Bauen und Umwelt e.V.) (Independent verifier)
1 Environmental Product Declaration ­ Dormakaba ­ ES 400 System ­ Sliding Door Operator
Product
Product description/Product definition
As a compact and innovative sliding door operator, the ES 400
is especially suitable for application in hospitals, institutes or
laboratories.
Thanks to its simple and low­maintenance design, it guarantees
easy handling and reliable function as well as a long life cycle.
The ES 410 effortlessly operates single­panel doors with a
weight of up to 200 kg at a passage width of up to 3 m, while
the ES 420 is especially suitable for double­panel doors with a
door­panel weight of up to 2x125 kg.
Features
• Compact design
• Excellent operating dynamics
• Applicable for heavy doors in stainless steel design
• Self­learning
• Parameterisation via software
• Push & Go function
• Separate input for control via fire detection system
• Integrated airlock function for up to 3 door sets
• Automatic changeover to manual closing For the placing on
the market in the European Union/European Free Trade
Product not harmonised in accordance with the CPR but in
Associaton (EU/EFTA) (with the exception of Switzerland) the
accordance with other provisions for harmonisation of the EU:
following legal provisions apply:
• DIN 18650:2010
• DIN 18650:2010
• DIN EN 16005: 2012
• DIN EN 16005: 2012
• DIN EN 60335-1, -2-103: 2007
• DIN EN 60335-1, -2-103: 2007
• DIN EN 61000-1-1:2017
• DIN EN 61000-1-2:2017
• DIN EN ISO 13849-1: 2016
• DIN EN ISO 13849-1: 2016
• DIN EN 61508-2: 2011
• DIN EN 61508-2: 2011
• 2011/65/EU ROHS3 Directive
• 2011/65/EU ROHS3 Directive
Delivery status:
The CE­marking takes into account the proof of conformity with
The declared ES 400 automatic drive system includes one
the respective harmonized standards based on the legal
average ES 400 (including one ES 420 drive unit kit double
provisions above.
leaf, one ES 400 slide rail complete 3m and one ES 400
adapter unit heavy load single leaf) and packaging with a
Application
weight of 18 kg.
Following parameter are applicable for single and double leaf
doors:
Base materials/Ancillary materials
The product composition of the ES 410/420 is as follows:
Technical Data
The technical specification of the ES 400 system is as follows:
The product contains partial articles which contain substances
listed in the Candidate List of REACH Regulation
1907/2006/EC (date: 17.01.2022) exceeding 0.1 percentage by
mass: no
Reference service life
The life cycle of the ES 400 drive system is about 5 years,
depending on the application and frequency of use. Regular
maintenance is advised to ensure the life expectancy of 5
years. For repairs or renewals, suitable spare parts are
available. The drive is tested to 200,000 cycles according to EN
2 Environmental Product Declaration ­ Dormakaba ­ ES 400 System ­ Sliding Door Operator
16005.
LCA: Calculation rules
Use stage - Module B6
Declared Unit The use stage related to the operation of the building includes:
The declared unit is 1 piece of the product: 16.6 kg — B6, operational energy use
Declared unit
End-of-life stage– Modules C1-C4 and D
Name Value Unit
The end­of­life stage includes:
Declared unit 1 pce.
— C1, de­construction, demolition:
Mass (total system) (excl. packaging) 16.6 kg — C2, transport to waste processing;
conversion factor 16.6 ­ — C3, waste processing for reuse, recovery and/or recycling;
— C4, disposal;
System boundary including provision and all transport, provision of all materials,
products and related energy and water use.
The type of EPD is: cradle to gate with options, modules C1–
C4, and module D (A1–A3 + C + D and additional modules: A4
Module D (Benefits and loads beyond the system boundary)
+ A5 + B6)
includes:
— D, recycling potentials, expressed as net impacts and
Production - Module A1-A3
benefits.
The product stage includes:
— A1, raw material extraction, processing and mechanical
Geographic Representativeness
treatments, processing of secondary material input (e.g.
Land or region, in which the declared product system is
recycling processes), — A2, transport to the manufacturer,
manufactured, used or handled at the end of the product´s
— A3, manufacturing and assembly including provision of all
lifespan: Germany
materials, products and energy, as well as waste processing up
to the end­of waste state.
Comparability
Construction stage - Modules A4-A5
Basically, a comparison or an evaluation of EPD data is only
The construction process stage includes:
possible if all the data sets to be compared were created
— A4, transport to the building site;
according to EN 15804 and the building context, respectively
— A5, installation into the building;
the product­specific characteristics of performance, are taken
including provision of all materials, products and energy, as well
into account. Background database: GaBi ts, SP40, CUP
as waste processing up to the end­of waste state or disposal of
2020.1
final residues during the construction process stage.
LCA: Scenarios and additional technical information
Reference service life
Characteristic product properties of biogenic carbon
Name Value Unit
Information on describing the Biogenic Carbon Content at
Life Span according to the manufacturer 5 a
factory gate
Name ValueUnit
kg
Biogenic carbon content in product 0.07
C Operational energy use (B6)
Biogenic carbon content in accompanying kg The use stage is declared for 5 years
0.52
packaging C Name Value Unit
Note: 1 kg of biogenic carbon is equivalent to 44/12 kg of CO . Electricity consumption for 1 year 199.75 kWh
2
Days per year in use 365 days
On mode per day 1.8 h
The following technical scenario information is required for the Idle mode per day 22.2 h
declared modules
On mode power 30.24 W
Transport from the gate to the site (A4)
Idle mode power 22.2 W
Name Value Unit
End of life (C1-C4)
Litres of fuel (per 1 kg) 0.00276 l/100km
Capacity utilisation (including empty runs) 55 % Name Value Unit
Transport distance via medium truck 100 km Recycling 15.86 kg
Energy recovery 0.56 kg
Transport distance is declared for a distance of 100km by truck
Landfilling 0.27 kg
in order to allow scaling to a specific point of installation.
Transport to waste management 50 km
Installation into the building (A5) The product is disassembled in a recycling process.
Name Value Unit Material recycling is then assumed for the metals, elec­tronic
and electromechanics. The plastic components are assumed to
Waste packaging (paper and plastic) 1.41 kg
be incinerated with energy recovery. Minor proportions of
residues arising from the recycling process are landfilled (1%).
3 Environmental Product Declaration ­ Dormakaba ­ ES 400 System ­ Sliding Door Operator
Region for the End of Life is: Global. scenario information
Collection rate is 100%.
Reuse, recovery and/or recycling potentials (D), relevant
4 Environmental Product Declaration ­ Dormakaba ­ ES 400 System ­ Sliding Door Operator
LCA: Results
Disclaimer:
EP­freshwater: This indicator has been calculated as 'kg P eq' as required in the characterization model (EUTREND model, Struijs et
al., 2009b, as implemented in ReCiPe; http://eplca.jrc.ec.europa.eu/LCDN/developerEF.xhtml).
DESCRIPTION OF THE SYSTEM BOUNDARY (X = INCLUDED IN LCA; MND = MODULE OR INDICATOR NOT DECLARED; MNR
= MODULE NOT RELEVANT)
Benefits and
Construction loads beyond
Product stage Use stage End of life stage
process stage the system
boundaries
la ire ta m w a Ry lp p u s tro p s n a rT g n iru tc a fu n a M e h t m o rf tro p s n a rTe tis e h t o t e ta g y lb m e s s A e s U e c n a n e tn ia M ria p e R tn e m e c a lp e R tn e m h s ib ru fe R y g re n e la n o ita re p Oe s u re ta w la n o ita re p Oe s u n o itc u rts n o c ­e Dn o itilo m e d tro p s n a rT g n is s e c o rp e ts a W la s o p s iD ­e s u e R­y re v o c e R­g n ilc y c e Rla itn e to p
A1 A2 A3 A4 A5 B1 B2 B3 B4 B5 B6 B7 C1 C2 C3 C4 D
X X X X X MND MND MNR MNR MNR X MND X X X X X
RESULTS OF THE LCA - ENVIRONMENTAL IMPACT according to EN 15804+A2: 1 piece ES 400 drive system
Parameter Unit A1-A3 A4 A5 B6 C1 C2 C3 C4 D
GWP­total kg CO 2 eq 4.86E+01 1.58E­01 2.02E+00 4.04E+02 0 7.28E­02 1.78E+00 2.93E­02 ­1.41E+01
GWP­fossil kg CO 2 eq 5.09E+01 1.51E­01 6.3E­02 4.02E+02 0 6.96E­02 1.43E+00 2.91E­02 ­1.41E+01
GWP­biogenic kg CO 2 eq ­2.22E+00 7E­03 1.96E+00 1.34E+00 0 3.22E­03 3.55E­01 9.95E­05 ­3.2E­02
GWP­luluc kg CO 2 eq 4.49E­02 3.6E­06 3.37E­05 5.83E­01 0 1.66E­06 8.36E­05 8.38E­05 ­3.99E­03
ODP kg CFC11 eq 1.37E­09 1.6E­17 3.68E­16 8.84E­12 0 7.34E­18 7.58E­16 1.08E­16 ­7.28E­11
AP mol H+ eq 2.2E­01 1.51E­04 5.65E­04 8.88E­01 0 6.96E­05 3.03E­04 2.09E­04 ­5.7E­02
EP­freshwater kg P eq 1.27E­04 3.24E­08 7.18E­08 1.07E­03 0 1.49E­08 1.2E­07 5E­08 ­8.35E­06
EP­marine kg N eq 3.68E­02 4.82E­05 2.04E­04 1.97E­01 0 2.22E­05 7.3E­05 5.38E­05 ­7.36E­03
EP­terrestrial mol N eq 3.97E­01 5.36E­04 2.54E­03 2.07E+00 0 2.46E­04 1.39E­03 5.91E­04 ­7.92E­02
kg NMVOC
POCP 1.14E­01 1.36E­04 5.4E­04 5.4E­01 0 6.26E­05 2.01E­04 1.63E­04 ­2.41E­02
eq
ADPE kg Sb eq 2.64E­03 4.54E­09 5.8E­09 1.16E­04 0 2.09E­09 1.05E­08 2.61E­09 ­3.11E­04
ADPF MJ 6.6E+02 2.15E+00 6.4E­01 7.07E+03 0 9.86E­01 7.33E­01 3.82E­01 ­1.89E+02
m3 world eq
WDP 6.23E+00 2.97E­04 2.5E­01 8.76E+01 0 1.36E­04 1.82E­01 3.05E­03 ­1.12E+00
deprived
GWP = Global warming potential; ODP = Depletion potential of the stratospheric ozone layer; AP = Acidification potential of land and water; EP =
Eutrophication potential; POCP = Formation potential of tropospheric ozone photochemical oxidants; ADPE = Abiotic depletion potential for non­fossil
resources; ADPF = Abiotic depletion potential for fossil resources; WDP = Water (user) deprivation potential)
RESULTS OF THE LCA - INDICATORS TO DESCRIBE RESOURCE USE according to EN 15804+A2: 1 piece ES 400 drive
system
Parameter Unit A1-A3 A4 A5 B6 C1 C2 C3 C4 D
PERE MJ 1.95E+02 6.77E­03 1.71E+01 3.13E+03 0 3.11E­03 2.78E+00 5E­02 ­6.79E+01
PERM MJ 1.96E+01 0 ­1.7E+01 0 0 0 ­2.59E+00 0 0
PERT MJ 2.15E+02 6.77E­03 1.17E­01 3.13E+03 0 3.11E­03 1.85E­01 5E­02 ­6.79E+01
PENRE MJ 6.45E+02 2.15E+00 8.55E­01 7.07E+03 0 9.87E­01 1.66E+01 3.82E­01 ­1.89E+02
PENRM MJ 1.6E+01 0 ­2.15E­01 0 0 0 ­1.58E+01 0 0
PENRT MJ 6.61E+02 2.15E+00 6.4E­01 7.07E+03 0 9.87E­01 7.33E­01 3.82E­01 ­1.89E+02
SM kg 1.13E+01 0 0 0 0 0 0 0 0
RSF MJ 0 0 0 0 0 0 0 0 0
NRSF MJ 0 0 0 0 0 0 0 0 0
FW m3 3.91E­01 1.21E­05 5.89E­03 3.62E+00 0 5.58E­06 4.34E­03 9.63E­05 ­1.33E­01
PERE = Use of renewable primary energy excluding renewable primary energy resources used as raw materials; PERM = Use of renewable primary
energy resources used as raw materials; PERT = Total use of renewable primary energy resources; PENRE = Use of non­renewable primary energy
excluding non­renewable primary energy resources used as raw materials; PENRM = Use of non­renewable primary energy resources used as raw
materials; PENRT = Total use of non­renewable primary energy resources; SM = Use of secondary material; RSF = Use of renewable secondary fuels;
NRSF = Use of non­renewable secondary fuels; FW = Use of net fresh water
RESULTS OF THE LCA – WASTE CATEGORIES AND OUTPUT FLOWS according to EN 15804+A2:
1 piece ES 400 drive system
Parameter Unit A1-A3 A4 A5 B6 C1 C2 C3 C4 D
HWD kg 2.76E­06 2.08E­10 9.57E­10 2.93E­06 0 9.58E­11 2.56E­09 5.82E­09 ­2.87E­06
NHWD kg 7.29E+00 2.2E­04 6.42E­02 5.02E+00 0 1.01E­04 1.5E­01 1.92E+00 ­2.3E+00
RWD kg 3.11E­02 2.31E­06 3.35E­05 1.07E+00 0 1.06E­06 2.87E­05 4.35E­06 ­1.65E­02
CRU kg 0 0 0 0 0 0 0 0 0
MFR kg 0 0 0 0 0 0 8.07E+00 0 0
MER kg 0 0 0 0 0 0 0 0 0
5 Environmental Product Declaration ­ Dormakaba ­ ES 400 System ­ Sliding Door Operator
EEE MJ 3.32E­01 0 3.06E+00 0 0 0 0 0 0
EET MJ 6.03E­01 0 5.56E+00 0 0 0 0 0 0
HWD = Hazardous waste disposed; NHWD = Non­hazardous waste disposed; RWD = Radioactive waste disposed; CRU = Components for re­use;
MFR = Materials for recycling; MER = Materials for energy recovery; EEE = Exported electrical energy; EET = Exported thermal energy
RESULTS OF THE LCA – additional impact categories according to EN 15804+A2-optional:
1 piece ES 400 drive system
Parameter Unit A1-A3 A4 A5 B6 C1 C2 C3 C4 D
Disease
PM 2.46E­06 7.96E­10 3.14E­09 7.44E­06 0 3.66E­10 3.48E­09 2.59E­09 ­8.25E­07
incidence
IR kBq U235 eq 5.11E+00 3.3E­04 5.17E­03 1.76E+02 0 1.51E­04 2.88E­03 4.47E­04 ­3.22E+00
ETP­fw CTUe 2.52E+02 1.52E+00 3.03E­01 3.02E+03 0 6.99E­01 2.8E­01 2.18E­01 ­6.02E+01
HTP­c CTUh 2.91E­07 2.86E­11 1.61E­11 8.35E­08 0 1.32E­11 2.36E­11 3.23E­11 ­3.68E­09
HTP­nc CTUh 7.88E­07 1.22E­09 7.09E­10 3.08E­06 0 5.63E­10 2.24E­09 3.56E­09 ­1.06E­07
SQP SQP 3.98E+02 5.52E­03 1.7E­01 2.25E+03 0 2.54E­03 2.18E­01 7.96E­02 ­8.5E+00
PM = Potential incidence of disease due to PM emissions; IR = Potential Human exposure efficiency relative to U235; ETP­fw = Potential comparative
Toxic Unit for ecosystems; HTP­c = Potential comparative Toxic Unit for humans (cancerogenic); HTP­nc = Potential comparative Toxic Unit for humans
(not cancerogenic); SQP = Potential soil quality index
Disclaimer 1 – for the indicator IRP
This impact category deals mainly with the eventual impact of low dose ionizing radiation on human health of the nuclear fuel cycle. It
does not consider effects due to possible nuclear accidents, occupational exposure nor radioactive waste disposal in underground
facilities. Potential ionizing radiation from the soil, from radon and from some construction materials is also not measured by this
indicator.
Disclaimer 2 – for the indicators ADPE, ADPF, WDP, ETP­fw, HTP­c, HTP­nc, SQP
The results of this environmental impact indicator shall be used with care as the uncertainties on these results are high or as there is
limited experience with the indicator.
References
Standards Directive 2011/65/EU of the European Parliament and of the
Council of 8 June 2011 on the restriction of the use of certain
DIN 18650 hazardous substances in electrical and electronic equipment
DIN 18650:2010, Powered pedestrian doors ­ Product
requirements and test methods IBU 2021
General Instructions for the EPD programme of Institut Bauen
DIN EN 60335 und Umwelt e.V.
DIN EN 60335­1, ­2­103:2020­08, Household and similar Version 2.0, Berlin: Institut Bauen und Umwelt e.V., 2021.
electrical appliances ­ Safety ­ Part 1: General requirements www.ibu­epd.com
DIN EN 61000 GaBi ts software
DIN EN 61000­1­2:2017­07, Electromagnetic compatibility Sphera Solutions GmbH Gabi Software System and Database
(EMC) ­ Part 1­2: General ­ Methodology for the achievement of for Life Cycle Engineering 1992­2020 Version 10.0.0.71
functional safety of electrical and electronic systems including University of Stuttgart Leinfelden­Echterdingen
equipment with regard to electromagnetic phenomena
GaBi ts documentation
DIN EN 61508 GaBi life cycle inventory data documentation
DIN EN 61508­2:2011­02, Functional safety of (https://www.gabisoftware.
electrical/electronic/programmable electronic safety­related com/support/gabi/gabidatabase­ 2020­lci­documentation/).
systems ­ Part 2: Requirements for
electrical/electronic/programmable electronic safety­related LCA-tool dormakaba
systems LCA tool, version 1.0. ENS (drive system)
Developed by Sphera Solutions GmbH.
DIN EN ISO 13849
DIN EN ISO 13849­1:2021­08, Safety of machinery ­ Safety­ PCR Part A
related parts of control systems ­ Part 1: General principles for PCR – Part A: Calculation Rules for the Life Cycle Assessment
design and Requirements on the Project Re­port according to EN
15804+A2:2019, Version 1.0, Institut Bauen und Umwelt e.V.,
EN 16005 www.ibu­epd.com.
DIN EN 16005: 2013­01, Power operated pedestrian doorsets ­
Safety in use ­ Requirements and test methods PCR Part B
PCR – Part B: Requirements on the EPD for Building Hardware
Further References product, version 1.2, Institut Bauen und Umwelt e.V., www.ibu­
epd.com, 2020.
2011/65/EU ROHS3 Directive
6 Environmental Product Declaration ­ Dormakaba ­ ES 400 System ­ Sliding Door Operator
Publisher
Institut Bauen und Umwelt e.V. +49 (0)30 3087748­ 0
Hegelplatz 1 info@ibu­epd.com
10117 Berlin www.ibu­epd.com
Germany
Programme holder
Institut Bauen und Umwelt e.V. +49 (0)30 3087748­ 0
Hegelplatz 1 info@ibu­epd.com
10117 Berlin www.ibu­epd.com
Germany
Author of the Life Cycle Assessment
Sphera Solutions GmbH +49 711 341817­0
Hauptstraße 111­ 113 info@sphera.com
70771 Leinfelden­Echterdingen www.sphera.com
Germany
Owner of the Declaration
dormakaba International Holding GmbH +49 2333 793­0
DORMA Platz 1 info.de@dormakaba.com
58256 Ennepetal www.dormakaba.com
Germany
7 Environmental Product Declaration ­ Dormakaba ­ ES 400 System ­ Sliding Door Operator
