ver1 2015
ENVIRONMENTAL PRODUCT DECLARATION
in accordance with ISO 14025, ISO 21930 and EN 15804
Owner of the declaration: ZENO-PROTECT B.V.
Program operator: The Norwegian EPD Foundation
Publisher: The Norwegian EPD Foundation
Declaration number: NEPD-2143-968-EN
Registration number: NEPD-2143-968-EN
ECO Platform reference number: -
Issue date: 17.04.2020
Valid to: 17.04.2025
EXCELLENCE
Zeno-Protect B.V.
www.epd-norge.no
NEPD-2143-968-EN EXCELLENCE
General information
Product: Owner of the declaration:
EXCELLENCE ZENO-PROTECT B.V.
Contact person: Pieter de Jong
Phone: +31 6 51 86 19 96
e-mail: pieter@zeno-protect.com
Program operator: Manufacturer:
The Norwegian EPD Foundation Mercury Flooring
Steenovenstraat 38
Pb. 5250 Majorstuen, 0303 Oslo B-8790 Waregem
BELGIUM
Phone: Phone: +47 977 22 020 Phone: +32 56 61 06 95
e-mail: post@epd-norge.no e-mail: info@mercuryflooring.com
Declaration number: Place of production:
NEPD-2143-968-EN Steenovenstraat 38
B-8790 Waregem
BELGIUM
ECO Platform reference number: Management system:
ISO 9001, ISO 14001
This declaration is based on Product Category Rules: Organisation no:
CEN Standard EN 15804 serves as core PCR NL805720819B01
This EPD is also compliant with IBU PCR for Building-
Related Products and Services, adapted for UL
Environment from the range of Environmental Product
Declarations of Institute Construction and Environment e.V.
(IBU), Part A: Calculation Rules for the Life Cycle
Assessment and Requirements on the Project report,
version 1.3 ) used in addition to the core PCR and IBU Part
B: Requirements on the EPD for Floor coverings.
Statement of liability: Issue date:
The owner of the declaration shall be liable for the 17.04.2020
underlying information and evidence. EPD Norway shall
not be liable with respect to manufacturerinformation, life
cycle assessment data and evidences.
Valid to:
17.04.2025
Declared unit: Year of study:
1 m² of synthetic entrance floor covering roll with a total 2019
weight of 4,2 kg
Declared unit with option: Comparability:
A1, A2, A3, A4, A5, C1,C2,C3,C4 EPD of construction products may not be comparable if they
not comply with EN 15804 and seen in a building context.
Functional unit: The EPD has been worked out by:
The EPD has been calculated by CO2logic team (Laura
Shahbenderian) using Open LCA software and EuGeos 15804-
IA Database Version 2.1
<sign>
Verification:
The CEN Norm EN 15804 serves as the core PCR.
Independent verification of the declaration and data,
according to ISO14025:2010
internal external
Approved
Third party verifier:
sign
<Harry van Ewijk MSc>
(Independent verifier approved by EPD Norway)
2/8
NEPD-2143-968-EN EXCELLENCE
Product
Product description: Technical data:
EXCELLENCE is a synthetic entrance floor covering made of Total product weight : 4,2 kg/m²
tufted polyamide with 100% of regenerated nylon, with a non- Pile weight: ca. 1 080 g/m²
woven recycled polyester primary backing and reinforced with Total height: ca. 8,7 mm
vinyl backing, manufactured by Zeno-Protect and designed to Pile height: ca. 6,7 mm
ensure the covering for heavy commercial use. Method of manufacture Tufted 5/32” cut pile
Pile material : 100% recycled ECONYL® nylon
EXCELLENCE Clean-Off-Zone is a distinction in the present Primary backing: Colback™ recycled polyester
ranges of products in this field, on account of an ingenuous Secondary backing: Comfort™ vinyl | Phthalate-Free
combination of small and larger polyamide filaments, resulting Number of tufts: ca. 92990 p/m²
in an optimal density. As a result dirt and moisture are more Use classification : 33, Commercial heavy
effectively stopped and contained. Dirt and moisture cannot Luxury comfort: LC3
spread into the building and avoids considerable cost in Suitable for castor chairs : A, intensive use r-3,1
cleaning. Suitable for stairs: Intensive use
Thermal resistance: 0,10 m² K/W
Also the spread of “fine dust” in the air will be prevented. This
will result in an improvement of the indoor air quality and The technical datasheet can be found on Zeno Protect
consequently in a reduction of the ill effects on health (the first brochure (page 2-3 for Excellence) :https://zeno-protect.com/wp-
step in fighting the Sick Building Syndrome). content/uploads/2019/11/Zeno-Protect-Clean-Off-
Zone_Brochure_2020_EN.pdf
Product specification: Market:
Global
Reference service life, product:
Materials kg % The service life of textile floorcoverings strongly depends on the
correct installation and the cleaning and maintenance instructions
provided by Zeno-Protect. The service life will vary depending on
the amount of floor traffic and the type and frequency of
Recycled nylon 0,9555 22,8 maintenance.
For Excellence, the Reference Service Life (RSL) of 10 years
could be assumed; technical service life can be considerably
longer.
Recycled polyester 0,0945 2,3
Polyvinyl chloride 1,0248 24,4 Reference service life, building:
Filler 0,798 19 60 years
Plasticizers 0,945 22,5
Additives 0,3822 9
LCA: Calculation rules
Declared unit: System boundary:
1 m² of synthetic entrance floor covering roll with a total The scope is a cradle to gate with options
weight of 4,2 kg (A1-A3, A4-A5,C1-C4)
3/8
NEPD-2143-968-EN EXCELLENCE
Data quality: Cut-off criteria:
Activity data is based on primary data collected amongst All major raw materials and all the essential energy is included.
Mercury Flooring (the manufacturer) for the year 2019 (energy, The production process for raw materials and energy flows that
waste, packaging, product components quantities, transport are included with very small amounts (<1%) are not included.
distances). Raw material stage data is derived directly from the This cut-off rule does not apply for hazardous materials and
Ecoinvent 3.3, cut-off database. substances.
Allocation:
The allocation is made ​​in accordance with the provisions of EN
15804. Incoming energy and water and waste production in-
house is allocated equally among all products through mass
allocation. Effects of primary production of recycled materials
allocated to the main product in which the material was used.
The recycling process and transportation of the material is
allocated to this analysis.
4/8
NEPD-2143-968-EN EXCELLENCE
LCA: Scenarios and additional technical information
The following information describe the scenarios in the different modules of the EPD.
This is a cradle to gate (A1-A3) EPD with no declared modules after the factory gate. Therefore this section is empty.
Transport from production place to user (A4)
Type Capacity utilisation (incl. return) Type of vehicle Distance km Fuel/Energy Value
% consumption (l/t)
Truck A4 63% Lorry 16-32 metric 209 0,038 l/tkm 7,8375
Truck A4 63% Lorry 16-32 metric 32,8 0,038 l/tkm 1,23
Truck C2 63% Lorry 16-32 metric 50 0,038 l/tkm 1,875
Truck for waste collection A5 50% 21 metric 50 0,336 l/tkm 16,8
Truck A4 68% Lorry 3.5-7.5 metric 202 0,109 l/tkm 22,018
Oceangoing ship A4 - Transoceanic ship 1133,5 ##### l/tkm 2,8338
The scenario for transport distances and transportation modes from manufacturing site to warehouse in Norway represents
both recorded and calculated routes and distances provided by N3Zones Group commercializing Protect Excellence
(Stopzoner) in Norway and Sweden. Transport in A4 describes the transport of the product from factory gate in Belgium to the
warehouse in Norway and transport to building in Norway/Sweden. Transportation of waste (A5, C2) is based on an average
distance of 50 km. Capacity utlization has been calculated by dividing the average load as reported in ecoinvent v3.3 by the
maximum load. Fuel consumption as given in ecoinvent v3.3.
Assembly (A5) Use (B1)
Unit Value Unit Value
Auxiliary kg 0,648
Water consumption m3
Electricity consumption kWh
Other energy carriers MJ
Material loss kg 0,756
Output materials from waste treatment kg
Dust in the air kg
<Short description>
Maintenance (B2)/Repair (B3) Replacement (B4)/Refurbishment (B5)
Unit Value Unit Value
Maintenance cycle* Replacement cycle*
Auxiliary kg Electricity consumption kWh
Other resources kg Replacement of worn parts 0
Water consumption m3
Electricity consumption kWh
Other energy carriers MJ
Material loss kg * Number or RSL (Reference Service Life)
<Short description>
Operational energy (B6) and water consumption (B7) End of Life (C1, C3, C4)
Unit Value Unit Value
Water consumption m3 Hazardous waste disposed kg
Electricity consumption kWh Collected as mixed construction waste kg
Other energy carriers MJ Reuse kg
Power output of equipment kW Recycling kg
Energy recovery kg 4,2
To landfill kg
Disposal is calculated as a municipal waste incineration scenario.
Transport to waste processing (C2)
Type Capacity utilisation (incl. return) Type of vehicle Distance km Fuel/Energy Value
% consumption (l/t)
0,038
Truck 63% Lorry 16-32 metric ton, EURO5 50 l/tkm 1,875
Railway kWh/tkm
Boat l/tkm
<Other Transportation> <xx>
Transport in C2 module is assumed to be made by a 16-32 road truck for an average distance of 50 km.
5/8
NEPD-2143-968-EN EXCELLENCE
<Short description>
Additional technical information
<Description>
LCA: Results
System boundaries (X=included, MND= module not declared, MNR=module not relevant)
Environmental impact
ecnanetniaM
esu
retaw
lanoitarepO
A5 B2 B4
X X
A5
tropsnarT
Unit
slairetam
waR
ylbmessA
Value
A1 A2 B6
X MND MND MNR MNR
riapeR
Benefits and loads beyond the system boundaries
(D)
Compared to previous version of EXCELLENCE, this product has been higly improved from environmental perspective. Indeed all impact
indicators have signgificantly decreased thanks to the use of 100% recycled nylon (pile material) and 100% recycled polyester (primary
backing). Table below shows the decreases for A1-A3 in % for LCA indicators compared to 2017:
B1
C2
kg CO -eqv 2
6,43E-09
tropsnarT
Parameter
tnemhsibrufeR
Use stage
MNR
esu
ygrene
lanoitarepO
B7
X MNR
A4
GWP
noitcurtsnoc-eD
noitilomed
C3
MND
tnemecalpeR
Beyond the
End of life stage system
boundaries
B5 C1 D
X X
1,12E+01 4,05E+00
kg CFC11-eqv 4,51E-07 1,39E-07
POCP 2,75E-03 5,69E-06
AP kg SO 2 -eqv 2,89E-02 3,13E-03 7,70E-03 0,00E+00 2,31E-03 0,00E+00
EP kg PO 43--eqv 8,14E-03 4,07E-04 1,79E-03 0,00E+00
ADPM kg Sb-eqv 3,75E-05 9,37E-06 1,15E-05 0,00E+00 3,32E-07 3,04E-06 0,00E+00
MJ
GWP Global warming potential; ODP Depletion potential of the stratospheric ozone layer; POCP Formation potential of tropospheric
photochemical oxidants; AP Acidification potential of land and water; EP Eutrophication potential; ADPM Abiotic depletion potential for non
fossil resources; ADPE Abiotic depletion potential for fossil resources
lasopsiD
-yrevoceR-esueR laitnetop-gnilcyceR
C4
X
C4
0,00E+00
0,00E+00
0,00E+00
gnissecorp
etsaW
C2
MND
C3
7,51E-08
tropsnarT
X X
8,72E+00
1,11E-04
1,81E-05 5,63E-04 0,00E+00
ADPE 1,96E+02 4,43E+01 5,19E-01 4,52E+00 0,00E+00
esU
A3 A4
gnirutcafunaM
Unit
Product stage Assemby stage
B3
A1- A3 C1
6,68E-01 0,00E+00 3,43E-02
ODP 1,18E-07 0,00E+00
kg C 2H 4 -eqv 1,44E-04 6,65E-04 0,00E+00 1,09E-04
9,91E+00 0,00E+00
6/8
NEPD-2143-968-EN EXCELLENCE
Resource use
Parameter Unit A1-A3 A4 A5 C1 C2 C3 C4
RPEE MJ 3,16E+01 1,61E-01 5,97E+00 0,00E+00 7,25E-03 3,31E-01 0,00E+00
RPEM MJ 0,00E+00 0,00E+00 0,00E+00 0,00E+00 0,00E+00 0,00E+00 0,00E+00
TPE MJ 3,16E+01 1,61E-01 5,97E+00 0,00E+00 7,25E-03 3,31E-01 0,00E+00
NRPE MJ 2,13E+02 1,06E+01 4,76E+01 0,00E+00 5,62E-01 4,56E+00 0,00E+00
NRPM MJ 8,25E+01 0,00E+00 0,00E+00 0,00E+00 0,00E+00 0,00E+00 0,00E+00
TRPE MJ 2,95E+02 1,06E+01 4,76E+01 0,00E+00 5,62E-01 4,56E+00 0,00E+00
SM kg 1,83E+00 0,00E+00 3,29E-01 0,00E+00 0,00E+00 1,34E-03 0,00E+00
RSF MJ 0,00E+00 0,00E+00 0,00E+00 0,00E+00 0,00E+00 0,00E+00 0,00E+00
NRSF MJ 6,13E-02 0,00E+00 1,10E-02 0,00E+00 0,00E+00 3,00E-03 0,00E+00
W m3 4,11E-01 2,03E-03 1,01E-01 0,00E+00 1,02E-04 9,36E-02 0,00E+00
RPEE Renewable primary energy resources used as energy carrier; RPEM Renewable primary energy resources used as raw materials; TPE
Total use of renewable primary energy resources; NRPE Non renewable primary energy resources used as energy carrier; NRPM Non
renewable primary energy resources used as materials; TRPE Total use of non renewable primary energy resources; SM Use of secondary
materials; RSF Use of renewable secondary fuels; NRSF Use of non renewable secondary fuels; W Use of net fresh water
End of life - Waste
Parameter Unit A1- A3 A4 A5 C1 C2 C3 C4
HW kg 2,41E-01 7,78E-03 1,46E-01 0,00E+00 2,98E-04 5,17E-01 0,00E+00
NHW kg 4,11E+00 5,75E-01 1,97E+00 0,00E+00 3,43E-02 4,67E+00 0,00E+00
RW kg 4,47E-04 6,83E-05 1,09E-04 0,00E+00 3,74E-06 2,07E-05 0,00E+00
HW Hazardous waste disposed; NHW Non hazardous waste disposed; RW Radioactive waste disposed
End of life - Output flow
Parameter Unit A1- A3 A4 A5 C1 C2 C3 C4
CR kg 0,00E+00 0,00E+00 0,00E+00 0,00E+00 0,00E+00 0,00E+00 0,00E+00
MR kg 3,53E-01 7,46E-03 7,21E-02 0,00E+00 3,41E-04 1,06E-02 0,00E+00
MER kg 0,00E+00 0,00E+00 0,00E+00 0,00E+00 0,00E+00 0,00E+00 0,00E+00
EEE MJ 1,97E+00 0,00E+00 0,00E+00 0,00E+00 0,00E+00 0,00E+00 0,00E+00
ETE MJ 0,00E+00 0,00E+00 0,00E+00 0,00E+00 0,00E+00 0,00E+00 0,00E+00
CR Components for reuse; MR Materials for recycling; MER Materials for energy recovery; EEE Exported electric energy; ETE Exported
thermal energy
Reading example: 9,0 E-03 = 9,0*10-3 = 0,009
Additional Norwegian requirements
Greenhous gas emission from the use of electricity in the manufacturing phase
National production mix from import, low woltage (production of transmission lines, in addition to direct emissions and losses in
grid) of applied electricity for the manufacturing prosess(A3).
Data source Amount Unit
Electricity, low voltage Belgium (market)
284,14 gCO-eqv/kWh
Econinvent v3.3 (2016), cut-off 2
Dangerous substances
The product contains no substances given by the REACH Candidate list or the Norwegian priority list
The product contains substances given by the REACH Candidate list or the Norwegian priority list that are less than 0,1 %
by weight.
The product contain dangerous substances, more then 0,1% by weight, given by the REACH Candidate List or the
Norwegian Priority list, see table.
The product contains no substances given by the REACH Candidate list or the Norwegian priority list. The product is
classified as hazardous waste (Avfallsforskiften, Annex III), see table.
7/8
NEPD-2143-968-EN EXCELLENCE
Name CAS no. Amount
Indoor environment
The product meets the requirements for low emissions (M1) according to EN15251: 2007 Appendix E.
Carbon footprint
Carbon footprint has not been worked out for the product.
Bibliography
ISO 14025:2010 Environmental labels and declarations - Type III environmental declarations - Principles and
procedures
ISO 14044:2006 Environmental management - Life cycle assessment - Requirements and guidelines
EN 15804:2012+A1:2013 Sustainability of construction works - Environmental product declaration - Core rules for the
product category of construction products
ISO 21930:2007 Sustainability in building construction - Environmental declaration of building products
LCA background report of Zeno protect products
IBU PCR for Building-Related Products and Services, adapted for UL Environment from the range of Environmental Product
Declarations of the Institute Construction and Environment e. V.
Ecoinvent database (v3.3)
Program operator Phone: +47 97722020
The Norwegian EPD Foundation
Post Box 5250, 030 Oslo e-mail: post@epd-norge.no
Norway web www.epd-norge.no
Publisher Phone: +47 97722020
The Norwegian EPD Foundation
Post Box 5250 Majorstuen, 0303 Oslo e-mail: post@epd-norge.no
Norway web www.epd-norge.no
Owner of the declaration Phone: +31651861996
Zeno-Protect B.V. Fax
Oostenburgervoorstraat 132, e-mail: pieter@zeno-protect.com
1018 MR Amsterdam, The Nederlands web www.zeno-protect.com
Author of the Life Cycle Assessment Phone: +32478413007
CO2logic Fax <xxxx>
Rue d'Accolay 15-17 e-mail: info@co2logic.com
1000, Brussels web www.co2logic.com
8/8
NEPD-2143-968-EN EXCELLENCE
