Environmental product declaration
in accordance with ISO 14025 and EN 15804+A2
Extruded PE 100 pipe and pipe systems
Owner of the declaration: Program operator:
AKVA group ASA The Norwegian EPD Foundation
Product: Declaration number:
Extruded PE 100 pipe and pipe systems
NEPD-6122-5391-EN
Declared unit:
1 kg Registration number:
This declaration is based on Product Category Rules: NEPD-6122-5391-EN
CEN Standard EN 15804:2012+A2:2019 serves as core
Issue date: 20.02.2024
PCR
The Norwegian EPD Foundation
NPCR Part A: Construction products and services Valid to: 20.02.2029
(application for plastic products)
EPD software:
LCAno EPD generator ID: 169481
1 / 11
General information
Product: Owner of the declaration:
Extruded PE 100 pipe and pipe systems AKVA group ASA
Contact person: Trude Olafsen
Phone: +47 91557400
e-mail: tolafsen@akvagroup.com
Program operator: Manufacturer:
Post Box 5250 Majorstuen, 0303 Oslo, Norway Helgeland Plast AS
The Norwegian EPD Foundation Båsmosjyen 4
Phone: +47 23 08 80 00 8616 Mo I Rana, Norway
web: post@epd-norge.no
Declaration number: Place of production:
AKVA group production site Mo i Rana (Norway)
NEPD-6122-5391-EN
Båsmosjyen 4
8616 Mo i Rana, Norway
This declaration is based on Product Category Rules: Management system:
CEN Standard EN 15804:2012+A2:2019 serves as core PCR AKVA group ASA sea-based nordic: ISO 9001:2015; Helgeland Plast:
NPCR Part A: Construction products and services (application for ISO 9001:2015 and ISO 14001:2015; Egersund Net AS: ISO
plastic products) 9001:2015 and ISO 14001:2015.
Statement of liability: Organisation no:
The owner of the declaration shall be liable for the underlying 931 693 670
information and evidence. EPD Norway shall not be liable with respect
to manufacturer information, life cycle assessment data and
evidences.​
Declared unit: Issue date: 20.02.2024
1 kg Extruded PE 100 pipe and pipe systems
Declared unit with option: Valid to: 20.02.2029
A1,A2,A3,A4,A5,C1,C2,C3,C4,D
Year of study:
2022
Functional unit: Comparability:
Not applicable. EPD of construction products may not be comparable if they not
comply with EN 15804 and seen in a building context.
General information on verification of EPD from EPD tools: Development and verification of EPD:
Independent verification of data, other environmental information The declaration is created using EPD tool lca.tools ver EPD2022.03,
and the declaration according to ISO 14025:2010, § 8.1.3 and § 8.1.4. developed by LCA.no. The EPD tool is integrated in the company's
Verification of each EPD is made according to EPD-Norway’s management system, and has been approved by EPD Norway.
guidelines for verification and approval requiring that tools are i)
integrated into the company's environmental management system, ii) Developer of EPD: Adrianne Mathea Løkås
the procedures for use of the EPD tool are approved by EPD-Norway,
Reviewer of company-specific input data and EPD:​ Elisabet Amat
and iii) the process is reviewed annually by an independent third
party verifier. See Appendix G of EPD-Norway's General Programme
Instructions for further information on EPD tools
Verification of EPD tool: Approved:
Independent third party verification of the EPD tool, background data
and test-EPD in accordance with EPDNorway's procedures and
guidelines for verification and approval of EPD tools. Approval
number: NEPDT68.
Third party verifier:
Elisabet Amat, GREENIZE projects
(no signature required)
2 / 11
Product:
Product description:
PE 100 Pipes and parts installed under ground, above ground, in water and in complete pipe systems for several industries. Appilicated for water
supply and drainage under pressure, non-pressure draines, sewers and surface water systems, aquaculture, land based fish farming and cable
protection.
Product specification:
PE 100, Polyethylene HDPE and packaging.
Materials kg %
Plastic - Polyethylene (HDPE) 1,00 100,00
Total 1,00
Packaging kg %
Packaging - HDPE parts 0,00 25,20
Packaging - Plastic straps 0,00 9,34
Packaging - Wood 0,00 65,45
Total incl. packaging 1,00
Technical data:
Production in accordance to EN 12201.
For more information, visit our website: https://www.akvagroup.com/sea-based/marine-infrastructure/pipes/
Market:
Norway.
Reference service life, product:
The service lifetime of the pipe or pipe system is at least 100 years, subject to relevant installation procedures being followed, and under normal
operations.
Reference service life, building or construction works:
Not relevant.
LCA: Calculation rules
Declared unit:
1 kg Extruded PE 100 pipe and pipe systems
Cut-off criteria:
All major raw materials and all the essential energy is included. The production processes for raw materials and energy flows with very small
amounts (less than 1%) are not included. These cut-off criteria do not​ apply for hazardous materials and substances.
Allocation:
The allocation is made in accordance with the provisions of EN 15804. Incoming energy and water and waste production in-house is allocated
equally among all products through mass allocation. Effects of primary production of recycled materials is allocated to the main product in which
the material was used. The recycling process and transportation of the material is allocated to this analysis.
Data quality:
Specific data for the product composition are provided by the manufacturer. The data represent the production of the declared product and were
collected for EPD development in the year of study. Background data is based on EPDs according to EN 15804 and different LCA databases. The
data quality of the raw materials in A1 is presented in the table below.
Materials Source Data quality Year
Packaging - HDPE parts ecoinvent 3.6 Database 2019
Packaging - Plastic straps ecoinvent 3.6 Database 2019
Packaging - Wood ecoinvent 3.6 Database 2019
Plastic - Polyethylene (HDPE) ecoinvent 3.6 Database 2019
3 / 11
System boundaries (X=included, MND=module not declared, MNR=module not relevant)
Construction Beyond the system
Product stage Use stage End of life stage
installation stage boundaries
A1 A2 A3 A4 A5 B1 B2 B3 B4 B5 B6 B7 C1 C2 C3 C4 D
X X X X X MND MND MND MND MND MND MND X X X X X
System boundary:
Additional technical information:
waR slairetam tropsnarT gnirutcafunaM tropsnarT ylbmessA e​sU ecnanetniaM riapeR tnemecalpeR tnemhsibrufeR lanoitarepO ygrene esu lanoitarepO esu retaw -eD noitcurtsnoc noitilomed tropsnarT etsaW gnissecorp lasopsiD -yrevoceR-esueR laitnetop-gnilcyceR
4 / 11
LCA: Scenarios and additional technical information
The following information describe the scenarios in the different modules of the EPD.
Module A4 = An average distance between the factory and the market is considered.
Module A5 = Installation activities are excluded from this EPD, only the waste treatment of packaging has been accounted for. This EPD has been
calculated per kg plastic pipes to cover a wide range of product dimensions. Contact Helgeland Plast to get a project/product specific EPD with
dimension specific installation results.
Module C1 = Excavation activities are excluded from this EPD. This EPD has been calculated per kg plastic pipes to cover a wide range of product
dimensions. Contact Helgeland Plast to get a project/product specific EPD with dimension specific de-construction results.
Module C2 = An average distance between the market and the waste treatment facility is considered.
Modules C3 and C4 = Waste treatments in C3 include material recycling and incineration with and without energy recovery and fly ash extraction.
Disposal in C4 consist of landfilling of different waste fractions and of ashes. In this EPD a conservative waste treatment scenario has been applied
with 50% of the plastic been sent to incineration with energy recovery and 50% being sent to landfilling.
Module D = The recyclability of plastics allows the producers a credit for the net scrap that is produced at the end of a product’s life. The benefits
from recycling of net scrap are described in formula from EN 15804:2012+A2:2019. Substitution of heat and electricity generated by the
incineration with energy recovery of plastics is also calculated in module D.
Capacity utilisation Value
Transport from production place to user (A4) Distance (km) Fuel/Energy Consumption Unit
(incl. return) % (Liter/tonne)
Truck, 16-32 tonnes, EURO 6 (km) - Europe 36,7 % 300 0,043 l/tkm 12,90
Assembly (A5) Unit Value
Waste, packaging, PET straps, to average
kg 0,00
treatment - A5 including transport (kg)
Waste, packaging, polyethylene, PE plastic parts,
to average treatment (kg) - A5 including transport kg 0,00
(kg)
Waste, packaging, wood to average treatment -
kg 0,00
A5 including transport (kg)
Capacity utilisation Value
Transport to waste processing (C2) Distance (km) Fuel/Energy Consumption Unit
(incl. return) % (Liter/tonne)
Truck, 16-32 tonnes, EURO 6 (km) - Europe 36,7 % 300 0,043 l/tkm 12,90
Waste processing (C3) Unit Value
Waste treatment of polyethylene (PE),
incineration with energy recovery and fly ash kg 0,50
extraction (kg)
Disposal (C4) Unit Value
Landfilling of ashes from incineration of
Polyethylene (PE), process per kg ashes and kg 0,02
residues (kg)
Landfilling of plastic mixture (kg) kg 0,50
Benefits and loads beyond the system
Unit Value
boundaries (D)
Substitution of electricity, in Norway (MJ) MJ 0,97
Substitution of thermal energy, district heating, in
MJ 14,67
Norway (MJ)
5 / 11
LCA: Results
The LCA results are presented below for the declared unit defined on page 2 of the EPD document.
Environmental impact
Indicator Unit A1 A2 A3 A4 A5 C1 C2 C3 C4 D
GWP-total
kg CO2 -
2,02E+00 1,23E-01 2,59E-02 4,90E-02 2,99E-03 0 4,90E-02 1,51E+00 5,81E-02 -8,81E-02
eq
GWP-fossil
kg CO2 -
2,01E+00 1,23E-01 2,48E-02 4,90E-02 1,29E-04 0 4,90E-02 1,51E+00 5,81E-02 -8,50E-02
eq
GWP-biogenic
kg CO2 -
7,63E-03 5,73E-05 9,95E-04 2,03E-05 2,86E-03 0 2,03E-05 1,22E-05 5,60E-06 -1,76E-04
eq
GWP-luluc
kg CO2 -
6,24E-04 6,75E-05 7,98E-05 1,74E-05 1,89E-08 0 1,74E-05 1,79E-06 1,26E-06 -2,93E-03
eq
kg
ODP CFC11 - 5,12E-08 2,36E-08 1,46E-09 1,11E-08 1,20E-11 0 1,11E-08 1,16E-09 1,66E-09 -6,20E-03
eq
mol H+
AP 7,21E-03 2,24E-03 1,56E-04 1,41E-04 5,02E-07 0 1,41E-04 1,89E-04 4,21E-05 -7,01E-04
-eq
EP-FreshWater kg P -eq 3,42E-05 1,20E-06 1,44E-06 3,92E-07 7,66E-10 0 3,92E-07 1,16E-07 6,45E-08 -7,56E-06
EP-Marine kg N -eq 1,23E-03 6,74E-04 1,91E-05 2,79E-05 2,62E-07 0 2,79E-05 9,07E-05 7,43E-05 -2,29E-04
mol N -
EP-Terrestial 1,38E-02 7,46E-03 2,34E-04 3,12E-04 2,21E-06 0 3,12E-04 9,81E-04 1,66E-04 -2,48E-03
eq
kg
POCP NMVOC 6,70E-03 1,97E-03 6,35E-05 1,19E-04 5,92E-07 0 1,19E-04 2,35E-04 5,93E-05 -6,83E-04
-eq
ADP- kg Sb-
1,80E-05 1,10E-06 1,44E-06 1,35E-06 1,23E-09 0 1,35E-06 5,28E-08 4,31E-08 -8,46E-07
minerals&metals1 eq
ADP-fossil1 MJ 7,09E+01 1,63E+00 2,79E-01 7,41E-01 9,15E-04 0 7,41E-01 9,87E-02 1,24E-01 -1,22E+00
WDP1 m3 7,49E+01 9,77E-01 4,54E+01 7,17E-01 2,05E-03 0 7,17E-01 2,23E-01 1,06E+00 -1,51E+01
GWP-total = Global Warming Potential total; GWP-fossil = Global Warming Potential fossil fuels; GWP-biogenic = Global Warming Potential biogenic; GWP-luluc =
Global Warming Potential land use and land use change; ODP = Depletion potential of the stratospheric ozone layer; AP = Acidification potential, Accumulated
Exceedance; EP-freshwater = Eutrophication potential, fraction of nutrients reaching freshwater end compartment: EP-marine = Eutrophication potential, fraction of
nutrients reaching marine end compartment; EP-terrestrial = Eutrophication potential, Accumulated Exceedance; POCP = Formation potential of tropospheric ozone;
ADP-minerals&metals = Abiotic depletion potential for non-fossil resources; ADP-fossil = Abiotic depletion for fossil resources potential; WDP = Water (user)
deprivation potential, deprivation-weighted water consumption
"Reading example: 9,0 E-03 = 9,0*10-3 = 0,009"
*INA Indicator Not Assessed
1. The results of this environmental impact indicator shall be used with care as the uncertainties on these results are high or as there is limited experienced with the
indicator
Remarks to environmental impacts:
6 / 11
Additional environmental impact indicators
Indicator Unit A1 A2 A3 A4 A5 C1 C2 C3 C4 D
PM Disease incidence 5,97E-08 8,83E-09 1,14E-09 3,00E-09 6,00E-12 0 3,00E-09 7,40E-10 8,24E-10 -4,25E-08
IRP2 kgBq U235 -eq 4,73E-02 6,89E-03 4,81E-03 3,24E-03 3,61E-06 0 3,24E-03 1,67E-04 5,96E-04 -7,77E-03
ETP-fw1 CTUe 1,11E+01 1,30E+00 1,21E+00 5,49E-01 9,82E-04 0 5,49E-01 2,95E-01 1,54E-01 -6,61E+00
HTP-c1 CTUh 5,42E-10 0,00E+00 5,90E-11 0,00E+00 0,00E+00 0 0,00E+00 3,40E-11 4,00E-12 -1,21E-10
HTP-nc1 CTUh 1,23E-08 1,71E-09 1,41E-09 6,00E-10 4,00E-12 0 6,00E-10 1,27E-09 1,19E-10 -6,34E-09
SQP1 dimensionless 2,38E+00 7,30E-01 1,38E-01 5,18E-01 8,95E-04 0 5,18E-01 1,20E-02 4,59E-01 -8,13E+00
PM = Particulate Matter emissions; IRP = Ionizing radiation – human health; ETP-fw = Eco toxicity – freshwater; HTP-c = Human toxicity – cancer effects; HTP-nc =
Human toxicity – non cancer effects; SQP = Potential Soil Quality Index (dimensionless)
"Reading example: 9,0 E-03 = 9,0*10-3 = 0,009"
*INA Indicator Not Assessed
1. The results of this environmental impact indicator shall be used with care as the uncertainties on these results are high or as there is limited experienced with the
indicator
2. This impact category deals mainly with the eventual impact of low dose ionizing radiation on human health of the nuclear fuel cycle. It does not consider effects due
to possible nuclear accidents, occupational exposure nor due to radioactive waste disposal in underground facilities. Potential ionizing radiation from the soil, from
radon and from some construction materials is also not measured by this indicator.
7 / 11
Resource use
Indicator Unit A1 A2 A3 A4 A5 C1 C2 C3 C4 D
PERE MJ 1,22E+00 3,05E-02 3,35E+00 1,06E-02 2,03E-05 0 1,06E-02 2,90E-03 5,83E-03 -7,51E+00
PERM MJ 2,62E-02 0,00E+00 0,00E+00 0,00E+00 -2,62E-02 0 0,00E+00 0,00E+00 0,00E+00 0,00E+00
PERT MJ 1,25E+00 3,05E-02 3,35E+00 1,06E-02 -2,62E-02 0 1,06E-02 2,90E-03 5,83E-03 -7,51E+00
PENRE MJ 3,15E+01 1,63E+00 2,79E-01 7,41E-01 9,15E-04 0 7,41E-01 9,87E-02 1,24E-01 -1,22E+00
PENRM MJ 4,25E+01 0,00E+00 0,00E+00 0,00E+00 -3,68E-02 0 0,00E+00 -4,23E+01 0,00E+00 0,00E+00
PENRT MJ 7,40E+01 1,63E+00 2,79E-01 7,41E-01 -3,58E-02 0 7,41E-01 -4,22E+01 1,24E-01 -1,22E+00
SM kg 2,74E-04 0,00E+00 0,00E+00 0,00E+00 0,00E+00 0 0,00E+00 0,00E+00 5,49E-05 0,00E+00
RSF MJ 7,07E-02 6,90E-04 2,79E-03 3,79E-04 5,69E-07 0 3,79E-04 8,17E-05 1,23E-04 -1,32E-03
NRSF MJ 8,99E-03 4,89E-03 6,74E-03 1,36E-03 4,60E-06 0 1,36E-03 0,00E+00 1,97E-03 -4,45E-01
FW m3 2,43E-02 2,01E-04 2,75E-02 7,92E-05 6,02E-07 0 7,92E-05 2,79E-04 1,51E-04 -9,05E-03
PERE = Use of renewable primary energy excluding renewable primary energy resources used as raw materials; PERM = Use of renewable primary energy resources used
as raw materials; PERT = Total use of renewable primary energy resources; PENRE = Use of non renewable primary energy excluding non-renewable primary energy
resources used as raw materials; PENRM = Use of non renewable primary energy resources used as raw materials; PENRT = Total use of non renewable primary energy
resources; SM = Use of secondary materials; RSF = Use of renewable secondary fuels; NRSF = Use of non-renewable secondary fuels; FW = Net use of fresh water
"Reading example: 9,0 E-03 = 9,0*10-3 = 0,009"
*INA Indicator Not Assessed
8 / 11
End of life - Waste
Indicator Unit A1 A2 A3 A4 A5 C1 C2 C3 C4 D
HWD kg 1,38E-03 1,12E-04 1,14E-03 3,82E-05 0,00E+00 0 3,82E-05 0,00E+00 1,49E-02 -5,72E-05
NHWD kg 6,39E-02 2,10E-02 2,22E-02 3,60E-02 2,86E-03 0 3,60E-02 0,00E+00 5,09E-01 -2,87E-02
RWD kg 4,22E-05 1,07E-05 2,43E-06 5,05E-06 0,00E+00 0 5,05E-06 0,00E+00 8,10E-07 -6,37E-06
HWD = Hazardous waste disposed; NHWD = Non-hazardous waste disposed; RWD = Radioactive waste disposed
"Reading example: 9,0 E-03 = 9,0*10-3 = 0,009"
*INA Indicator Not Assessed
End of life - Output flow
Indicator Unit A1 A2 A3 A4 A5 C1 C2 C3 C4 D
CRU kg 0,00E+00 0,00E+00 0,00E+00 0,00E+00 0,00E+00 0 0,00E+00 0,00E+00 0,00E+00 0,00E+00
MFR kg 0,00E+00 0,00E+00 7,56E-03 0,00E+00 5,05E-04 0 0,00E+00 0,00E+00 4,48E-05 0,00E+00
MER kg 0,00E+00 0,00E+00 7,12E-03 0,00E+00 1,87E-03 0 0,00E+00 5,00E-01 1,10E-06 0,00E+00
EEE MJ 0,00E+00 0,00E+00 5,49E-03 0,00E+00 1,31E-03 0 0,00E+00 9,70E-01 7,12E-05 0,00E+00
EET MJ 0,00E+00 0,00E+00 8,30E-02 0,00E+00 1,98E-02 0 0,00E+00 1,47E+01 1,08E-03 0,00E+00
CRU = Components for re-use; MFR = Materials for recycling; MER = Materials for energy recovery; EEE = Exported energy electrical; EET = Exported energy thermal
"Reading example: 9,0 E-03 = 9,0*10-3 = 0,009"
*INA Indicator Not Assessed
Biogenic Carbon Content
Indicator Unit At the factory gate
Biogenic carbon content in product kg C 0,00E+00
Biogenic carbon content in accompanying packaging kg C 7,80E-04
Note: 1 kg biogenic carbon is equivalent to 44/12 kg CO2
9 / 11
Additional requirements
Greenhouse gas emissions from the use of electricity in the manufacturing phase:
National production mix from import, low voltage (production of transmission lines, in addition to direct emissions and losses in grid) of applied
electricity for the manufacturing process (A3).
Electricity mix Data source Amount Unit
Electricity, Norway (kWh) ecoinvent 3.6 24,33 g CO2-eq/kWh
Dangerous substances:
The product contains no substances given by the REACH Candidate list.
Indoor environment:
Additional Environmental Information
Additional environmental impact indicators required in NPCR Part A for construction products
Indicator Unit A1 A2 A3 A4 A5 C1 C2 C3 C4 D
GWPIOBC kg CO2 -eq 1,90E+00 1,23E-01 2,58E-02 4,90E-02 1,29E-04 0 4,90E-02 1,51E+00 5,81E-02 -8,69E-02
GWP-IOBC: Global warming potential calculated according to the principle of instantaneous oxidation. In order to increase the transparency of biogenic carbon​
contribution to climate impact, the indicator GWP-IOBC is required as it declares climate impacts calculated according to the principle of instantaneous oxidation.​
GWP-IOBC is also referred to as GWP-GHG in context to Swedish public procurement legislation.
10 / 11
Bibliography
ISO 14025:2010 Environmental labels and declarations - Type III environmental declarations - Principles and procedures.
ISO 14044:2006 Environmental management - Life cycle assessment - Requirements and guidelines.
EN 15804:2012+A2:2019 Environmental product declaration - Core rules for the product category of construction products.
ISO 21930:2017 Sustainability in buildings and civil engineering works - Core rules for environmental product declarations of construction
products.
ecoinvent v3, Allocation, cut-off by classification, Swiss Centre of Life Cycle Inventories.
Iversen et al., (2021) eEPD v2021.09 Background information for EPD generator tool system verification, LCA.no Report number: 07.21
Graafland, J. and Ruttenborg, M. (2023) EPD generator for Plastic products, Background information for EPD generator application and LCA data,
LCA.no report number: 06.23
NPCR Part A: Construction products and services. Ver. 2.0. March 2021, EPD-Norge.
Data for EPD originated from BOM and actual consumptions of reference year.
Program operator and publisher: Phone: +47 23 08 80 00
The Norwegian EPD Foundation e-mail: post@epd-norge.no
Post Box 5250 Majorstuen, 0303 Oslo, Norway web: www.epd-norge.no
Owner of the declaration: Phone: +47 91557400
AKVA group ASA e-mail: tolafsen@akvagroup.com
Plogfabrikkvegen 11, 4353 Klepp Stasjon web: https://www.akvagroup.com
Author of the Life Cycle Assessment: Phone: +47 916 50 916
LCA.no AS e-mail: post@lca.no
Dokka 6B, 1671 web: www.lca.no
Developer of EPD generator: Phone: +47 916 50 916
LCA.no AS e-mail: post@lca.no
Dokka 6B,1671 Kråkerøy web: www.lca.no
ECO Platform web: www.eco-platform.org
ECO Portal web: ECO Portal
11 / 11
