ENVIRONMENTAL PRODUCT DECLARATION
as per ISO 14025 and EN 15804+A2
Owner of the Declaration VELUX Group
Publisher Institut Bauen und Umwelt e.V. (IBU)
Programme holder Institut Bauen und Umwelt e.V. (IBU)
Declaration number EPD-VEL-20230051-IBA2-EN
Issue date 11.05.2023
Valid to 10.05.2028
Window operator for VELUX pivot hinged windows (KMG 100K)
and control system (KUX 110), mains connected
VELUX Group
www.ibu-epd.com | https://epd-online.com
General Information
VELUX Group Window operator for VELUX pivot hinged windows
(KMG 100K) and control system (KUX 110), mains
connected
Programme holder Owner of the declaration
IBU – Institut Bauen und Umwelt e.V. VELUX Group
Hegelplatz 1 Ådalsvej 99
10117 Berlin 2970 Hørsholm
Germany Denmark
Declaration number Declared product / declared unit
EPD-VEL-20230051-IBA2-EN The declared unit is one piece of electrical window operator.
This declaration is based on the product category rules: Scope:
Drive systems for automatic doors and gates, 01.08.2021 The EPD is a specific EPD covering VELUX electrical window operator for
(PCR checked and approved by the SVR) the mains connected pivot hinged windows. The operator consists of a
chain operator, a rain sensor, a control system and a remote. The products
are manufactured by the VELUX Group at a production site in the Czech
Issue date Republic.
The owner of the declaration shall be liable for the underlying information
11.05.2023
and evidence; the IBU shall not be liable with respect to manufacturer
information, life cycle assessment data and evidences.
Valid to
The EPD was created according to the specifications of EN 15804+A2. In
10.05.2028 the following, the standard will be simplified as EN 15804.
Verification
The standard EN 15804 serves as the core PCR
Independent verification of the declaration and data according to ISO
14025:2011
internally X externally
Dipl.-Ing. Hans Peters
(Chairman of Institut Bauen und Umwelt e.V.)
Florian Pronold Dr.-Ing. Nikolay Minkov,
(Managing Director Institut Bauen und Umwelt e.V.) (Independent verifier)
1 Environmental Product Declaration - VELUX Group - Window operator for VELUX pivot hinged windows (KMG 100K) and control system (KUX 110), mains connected
Product
Product description/Product definition Base materials/Ancillary materials
EPD covering VELUX electrical window operator for the mains
Product content
connected pivot hinged windows. The operator consists of a
Name Value Unit
chain operator, a rain sensor, a control system and a remote.
The products are manufactured by the VELUX Group at a Other plastic components 34 %
production site in the Czech Republic. Cables 20 %
For the placing on the market of the product in the European Other metal components 16 %
Union/European Free Trade Association (EU/EFTA) (with the
PCBA 6 %
exception of Switzerland) Regulation (EU) No. 305/2011 (CPR)
Motor 4 %
applies. The products are in compliance with the Machinery
Directive 2006/42/EC, the Radio Equipment Directive Battery 1 %
2014/53/EU and the RoHS Directive 2011/65/EU. A declaration Other (butyl sealant, epoxy, paper) 18 %
of conformity is available from the manufacturer.
Packaging materials include 0,46 kg cardboard and paper, 0,14
kg polystyren (EPS) and 0,03 kg low density polyethylen
Application
(LDPE) per declared unit.
The VELUX electrical window operator is sold separately for
retrofitting.
This product/article/at least one partial article contains
Technical Data substances listed in the candidate list (date: 08.06.2022)
exceeding 0.1 percentage by mass: NO.
The CE marking for electrical window operators does not
specify the need for a Declaration of Performance. Instead, a
Reference service life
Declaration of Conformity is required.
No reference service life (RSL) is defined for the operators as
The performance values relevant for the product are specified
the use stage modules are not included in the EPD. There is no
in the table below.
generally acknowledged or common way to assess the RSL for
Constructional data this type of product. Furthermore, the lifetime of the products
Name Value Unit depends greatly on the use pattern and environmental
conditions in use, which differs for different users and which is
Protection class IP 44 class
difficult to predict at the time of sale.
Voltage 230 V
LCA: Calculation rules
A3 - Manufacturing: The products are produced/assembled at
Declared Unit the VELUX production site, where the finished window operator
The declared unit is one piece. This corresponds to an is ready for shipment.
electrical window operator system, including a chain operator, a
control system, a rain sensor and a remote. End of life stage:
Name Value Unit
Declared unit 1 pce. C1 - De-construction/demolition: de-construction of the product
with the use of manual hand tools.
Weight 1,93 kg
Conversion factor to kg 0,52 -
C2 - Transport: transport of the product to waste treatment
Other declared units are allowed if the conversion is shown including to and from sorting and shredding facilities.
transparently.
C3 - Waste processing: includes sorting, shredding, incineration
A data quality and a sensitivity analysis show that the results and recycling processes.
are robust with regard to data quality and appropriateness.
There is low variability of production processes and product C4 - Disposal: disposal of all materials
variations have a limited influence on the results.
Benefits and loads beyond the system boundaries:
System boundary
Type of EPD: D - Reuse, recovery and recycling potential: benefits from
Cradle to gate - with options. The following life cycle phases plastic incineration processes and material recycling. End of life
were considered: includes all activities from when the product reaches the end of
its service life and no longer provides any functionality until all
Product stage: materials and components are processed for
reuse/recycling/energy recovery or are disposed of.
A1 - Raw material supply: extraction and processing,
production of the pre-products (e.g. motor suspension, PCB, The applied end-of-life scenario follows the requirements in the
battery...). Production of packaging: cardboard boxes, paper PCR Part A, chapter 6.2 regarding complex products, with a
labels, EPS and plastic film. combination of recycling, thermal waste treatment and
landfilling. 100% of the material is considered in the end-of-life
A2 - Transport: Transport of pre-products and packaging scenario. Generally metals, cables, batteries and
components to the manufacturing sites. polychlorinated biphenyl (PCB)'s are recycled, plastic parts are
incinerated with energy recovery and magnets are landfilled.
2 Environmental Product Declaration - VELUX Group - Window operator for VELUX pivot hinged windows (KMG 100K) and control system (KUX 110), mains connected
Basically, a comparison or an evaluation of EPD data is only
Geographic Representativeness possible if all the data sets to be compared were created
Land or region, in which the declared product system is according to EN 15804 and the building context, respectively
manufactured, used or handled at the end of the product´s the product-specific characteristics of performance, are taken
lifespan: Europe into account. The used background software and database is
GaBi (DB version 2021.2)
Comparability
LCA: Scenarios and additional technical information
No Reference Service Life (RFL) is declared, because the use
Characteristic product properties of biogenic carbon stage modules are not declared.
The product does not contain biogenic carbon.
End of life (C1-C4)
Information on describing the biogenic Carbon Content at
Name Value Unit
factory gate
Collected separately waste type Electronics 1.9 kg
Name ValueUnit
Recycling 0.89 kg
kg
Biogenic carbon content in product - Energy recovery 1.01 kg
C
Landfilling 0.03 kg
Biogenic carbon content in accompanying kg
0.37
packaging C
Reuse, recovery and/or recycling potentials (D), relevant
scenario information
Name Value Unit
Assembly (A5) Replaced materials 0.18 kg
Name Value Unit Replaced thermal energy 4.8 MJ
Cardboard for recycling 0.46 kg Replaced electricity 2.6 MJ
EPS packaging for incineration 0.14 kg
Plastic packaging for incineration (LDPE) 0.03 kg
3 Environmental Product Declaration - VELUX Group - Window operator for VELUX pivot hinged windows (KMG 100K) and control system (KUX 110), mains connected
LCA: Results
DESCRIPTION OF THE SYSTEM BOUNDARY (X = INCLUDED IN LCA; MND = MODULE OR INDICATOR NOT DECLARED; MNR
= MODULE NOT RELEVANT)
Benefits and
Construction loads beyond
Product stage Use stage End of life stage
process stage the system
boundaries
la ire ta m w a Ry lp p u s tro p s n a rT g n iru tc a fu n a M e h t m o rf tro p s n a rTe tis e h t o t e ta g y lb m e s s A e s U e c n a n e tn ia M ria p e R tn e m e c a lp e R tn e m h s ib ru fe R y g re n e la n o ita re p Oe s u re ta w la n o ita re p Oe s u n o itc u rts n o c -e Dn o itilo m e d tro p s n a rT g n is s e c o rp e ts a W la s o p s iD -e s u e R-y re v o c e R-g n ilc y c e Rla itn e to p
A1 A2 A3 A4 A5 B1 B2 B3 B4 B5 B6 B7 C1 C2 C3 C4 D
X X X MND MND MND MND MNR MNR MNR MND MND X X X X X
RESULTS OF THE LCA - ENVIRONMENTAL IMPACT according to EN 15804+A2: 1 pcs window operator
Parameter Unit A1 A2 A3 C1 C2 C3 C4 D
GWP-total kg CO 2 eq 1.15E+01 4.49E-01 7.33E-01 0 8.85E-03 1.67E+00 1.47E-05 -1.36E+00
GWP-fossil kg CO 2 eq 1.16E+01 4.48E-01 1.36E+00 0 8.79E-03 1.67E+00 1.51E-05 -1.36E+00
GWP-biogenic kg CO 2 eq -1.32E-01 1.89E-04 -6.28E-01 0 -1.12E-05 1.28E-03 -4.39E-07 -5.41E-04
GWP-luluc kg CO 2 eq 1.62E-02 1.25E-03 1.19E-03 0 7.19E-05 1.79E-04 4.44E-08 -1.54E-03
ODP kg CFC11 eq 1.37E-09 4.98E-17 1.95E-11 0 1.12E-18 6.17E-09 5.88E-20 -8.13E-15
AP mol H+ eq 5.13E-02 1.13E-02 4.07E-03 0 2.75E-05 1.9E-03 1.08E-07 -4.21E-03
EP-freshwater kg P eq 1.59E-04 5.16E-07 1.56E-05 0 2.61E-08 1.03E-05 2.54E-11 -1.36E-06
EP-marine kg N eq 8.78E-03 3.09E-03 1.29E-03 0 1.26E-05 8.79E-04 2.8E-08 -7.15E-04
EP-terrestrial mol N eq 9.27E-02 3.39E-02 1.31E-02 0 1.41E-04 9.69E-03 3.07E-07 -7.7E-03
kg NMVOC
POCP 2.77E-02 8.46E-03 3.78E-03 0 2.47E-05 2.25E-03 8.47E-08 -2.13E-03
eq
ADPE kg Sb eq 8.84E-04 2.04E-08 2.01E-07 0 6.69E-10 2.08E-07 1.43E-12 -4.03E-05
ADPF MJ 1.77E+02 5.6E+00 2.73E+01 0 1.17E-01 2.48E+00 2.01E-04 -1.9E+01
m3 world eq
WDP 4.88E+00 1.77E-03 1.67E-01 0 7.63E-05 5.03E-01 1.62E-06 -2.7E-01
deprived
GWP = Global warming potential; ODP = Depletion potential of the stratospheric ozone layer; AP = Acidification potential of land and water; EP =
Eutrophication potential; POCP = Formation potential of tropospheric ozone photochemical oxidants; ADPE = Abiotic depletion potential for non-fossil
resources; ADPF = Abiotic depletion potential for fossil resources; WDP = Water (user) deprivation potential)
RESULTS OF THE LCA - INDICATORS TO DESCRIBE RESOURCE USE according to EN 15804+A2: 1 pcs window operator
Parameter Unit A1 A2 A3 C1 C2 C3 C4 D
PERE MJ 2.94E+01 1.25E-01 1.73E+01 0 6.53E-03 7.77E-01 2.7E-05 -4.05E+00
PERM MJ 0 0 0 0 0 0 0 0
PERT MJ 2.94E+01 1.25E-01 1.73E+01 0 6.53E-03 7.77E-01 2.7E-05 -4.05E+00
PENRE MJ 1.53E+02 5.61E+00 1.91E+01 0 1.17E-01 2.01E+01 2.01E-04 -1.9E+01
PENRM MJ 2.33E+01 0 8.24E+00 0 0 -1.76E+01 0 0
PENRT MJ 1.77E+02 5.61E+00 2.73E+01 0 1.17E-01 2.48E+00 2.01E-04 -1.9E+01
SM kg 1.79E-01 0 0 0 0 0 0 0
RSF MJ 0 0 0 0 0 0 0 0
NRSF MJ 0 0 0 0 0 0 0 0
FW m3 1.29E-01 1.49E-04 7.85E-03 0 7.47E-06 1.21E-02 4.95E-08 -1.13E-02
PERE = Use of renewable primary energy excluding renewable primary energy resources used as raw materials; PERM = Use of renewable primary
energy resources used as raw materials; PERT = Total use of renewable primary energy resources; PENRE = Use of non-renewable primary energy
excluding non-renewable primary energy resources used as raw materials; PENRM = Use of non-renewable primary energy resources used as raw
materials; PENRT = Total use of non-renewable primary energy resources; SM = Use of secondary material; RSF = Use of renewable secondary fuels;
NRSF = Use of non-renewable secondary fuels; FW = Use of net fresh water
RESULTS OF THE LCA – WASTE CATEGORIES AND OUTPUT FLOWS according to EN 15804+A2:
1 pcs window operator
Parameter Unit A1 A2 A3 C1 C2 C3 C4 D
HWD kg 2.58E-04 1.3E-10 1.35E-04 0 5.9E-12 5.5E-10 2.13E-14 -2.97E-09
NHWD kg 6.17E-01 6.6E-04 3.61E-02 0 1.74E-05 1.23E-01 1E-03 -5.13E-02
RWD kg 3.17E-03 6.43E-06 1.33E-03 0 1.42E-07 2.29E-04 2.11E-09 -9.03E-04
CRU kg 0 0 0 0 0 0 0 0
MFR kg 0 0 0 0 0 6.96E-01 0 0
MER kg 0 0 0 0 0 6.71E-01 0 0
EEE MJ 0 0 0 0 0 0 0 2.63E+00
EET MJ 0 0 0 0 0 0 0 4.75E+00
4 Environmental Product Declaration - VELUX Group - Window operator for VELUX pivot hinged windows (KMG 100K) and control system (KUX 110), mains connected
HWD = Hazardous waste disposed; NHWD = Non-hazardous waste disposed; RWD = Radioactive waste disposed; CRU = Components for re-use;
MFR = Materials for recycling; MER = Materials for energy recovery; EEE = Exported electrical energy; EET = Exported thermal energy
RESULTS OF THE LCA – additional impact categories according to EN 15804+A2-optional:
1 pcs window operator
Parameter Unit A1 A2 A3 C1 C2 C3 C4 D
Disease
PM 6.66E+01 3.94E+00 9.61E+00 0 8.21E-02 9.99E+00 1.07E-04 -4.29E+00
incidence
IR kBq U235 eq 3.58E+01 6.94E-02 2.41E+01 0 1.59E-03 1.57E+00 6.15E-06 -1.91E+00
ETP-fw CTUe 4.36E-01 3.58E-02 8.08E-02 0 7.89E-04 5.79E-02 8.69E-07 -4.31E-02
HTP-c CTUh 2.85E-19 1.33E-21 5.91E-20 0 2.93E-23 5.92E-20 1.85E-25 -2.53E-19
HTP-nc CTUh 3.83E-09 7.6E-11 1.96E-10 0 1.67E-12 7.89E-10 1.64E-14 -8.92E-10
SQP SQP 7.45E-08 1.71E-12 9.33E-11 0 3.9E-14 2.74E-11 4.93E-16 -3.85E-10
PM = Potential incidence of disease due to PM emissions; IR = Potential Human exposure efficiency relative to U235; ETP-fw = Potential comparative
Toxic Unit for ecosystems; HTP-c = Potential comparative Toxic Unit for humans (cancerogenic); HTP-nc = Potential comparative Toxic Unit for humans
(not cancerogenic); SQP = Potential soil quality index
Disclaimer 1 – for the indicator 'Potential Human exposure efficiency relative to U235'. This impact category deals mainly with the
eventual impact of low dose ionizing radiation on human health of the nuclear fuel cycle. It does not consider effects due to possible
nuclear accidents, occupational exposure or radioactive waste disposal in underground facilities. Potential ionizing radiation from the
soil, radon and from some construction materials is also not measured by this indicator.
Disclaimer 2 – for the indicators 'abiotic depletion potential for non-fossil resources', 'abiotic depletion potential for fossil resources',
'water (user) deprivation potential, deprivation-weighted water consumption', 'potential comparative toxic unit for ecosystems', 'potential
comparative toxic unit for humans – cancerogenic', 'Potential comparative toxic unit for humans - not cancerogenic', 'potential soil
quality index'. The results of this environmental impact indicator shall be used with care as the uncertainties on these results are high
as there is limited experience with the indicator.
References
IBU PCR Part A Council, 17 May 2006 on Machinery.
IBU PCR Part A: Institut Bauen und Umwelt e.V., Product
Category Rules for Building-Related Products and Services. DIN EN ISO 14025:2011-10
Calculation Rules for the Life Cycle Assessment and DIN EN ISO 14025:2011-10, Environmental labels and
Requirements on the Project Report according to EN declarations - Type III environmental declarations - Principles
15804+A2:2019. and procedures.
IBU PCR Part B: EN 14351-1:2006+A2:2016
IBU PCR Part B: Institut Bauen und Umwelt e.V., Requirements EN14351-1:2006+A2:2016, Windows and doors - Product
on the EPD for Drive systems for automatic doors and gates, standard, performance characteristics - Part 1: Windows and
version 1.6. external pedestrian doorsets.
IBU 2021 EN 15804:2019+A2
IBU 2021 Institut Bauen und Umwelt e.V.: General Instructions EN15804:2019+A2: Sustainability of construction works -
for the EPD programme of Institut Bauen und Umwelt e.V. Environmental Product Declarations - Core rules for the product
Version 2.0, Berlin: Institut Bauen und Umwelt e.V., 2021. category of construction products.
www.ibu-epd.com.
Directive 2014/53/EU
EN 13501-1 Directive 2014/53/EU of the European Parliament and of the
EN13501-1, 2018: Fire classification of construction products Council of 16 April 2014 on the harmonisation of the laws of the
and building elements - Part 1: Classification using data from Member States relating to the making available on the market
reaction to fire tests. of radio equipment.
Directive 2014/53/EU Directive 2011/65/EU
Directive 2014/53/EU of the European Parliament and of the Directive 2011/65/EU of the European Parliament and of the
Council, 16 April 2014, on harmonisation of the laws of the Council of 8 June 2011 on the restriction of the use of certain
Member States relating to the making available on the market hazardous substances in electrical and electronic equipment.
of radio equipment.
Directive 2006/42/EC
Regulation (EU) No 305/2011 DIRECTIVE 2006/42/EC OF THE EUROPEAN PARLIAMENT
Regulation (EU) No 305/2011 of the European Parliament and AND OF THE COUNCIL of 17 May 2006 on machinery.
of the Council, 9 March 2011, Laying down harmonised
conditions for the marketing of constructional products. Candidate list
Candidate List of substances of very high concern for
Directive 2011/65/EU Authorisation, 08.06.2022.
Directive 2011/65/EU of the European Parliament and of the
Council, 8 June 2011, on the restriction of the use of certain GaBi LCA software and database
hazardous substances in electrical and electronic equipment. The LCA modelling software is GaBi program version
10.5.1.124 with corresponding databases from Sphera
Directive 2006/42/EC Solutions GmbH. Documentation hyperlink www.gabi-
Directive 2006/42/EC of the European Parliament and of the software.com/support/gabi.
5 Environmental Product Declaration - VELUX Group - Window operator for VELUX pivot hinged windows (KMG 100K) and control system (KUX 110), mains connected
6 Environmental Product Declaration - VELUX Group - Window operator for VELUX pivot hinged windows (KMG 100K) and control system (KUX 110), mains connected
Publisher
Institut Bauen und Umwelt e.V. +49 (0)30 3087748- 0
Hegelplatz 1 info@ibu-epd.com
10117 Berlin www.ibu-epd.com
Germany
Programme holder
Institut Bauen und Umwelt e.V. +49 (0)30 3087748- 0
Hegelplatz 1 info@ibu-epd.com
10117 Berlin www.ibu-epd.com
Germany
Author of the Life Cycle Assessment
FORCE Technology +4543250856
Park Alle 345 chme@force.dk
2605 Brøndby www.forcetechnology.com
Denmark
Owner of the Declaration
VELUX Group +4545164726
Ådalsvej 99 jakob.roerbech@velux.com
2970 Hørsholm www.velux.com
Denmark
7 Environmental Product Declaration - VELUX Group - Window operator for VELUX pivot hinged windows (KMG 100K) and control system (KUX 110), mains connected
