ENVIRONMENTAL PRODUCT DECLARATION
as per ISO 14025 and EN 15804+A2
Owner of the Declaration VELUX Group
Publisher Institut Bauen und Umwelt e.V. (IBU)
Programme holder Institut Bauen und Umwelt e.V. (IBU)
Declaration number EPD-VEL-20220111-CBB3-EN
Issue date 24.05.2022
Valid to 23.05.2027
Collar BFX
Velux
www.ibu-epd.com | https://epd-online.com
General Information
Velux Collar BFX
Programme holder Owner of the declaration
IBU – Institut Bauen und Umwelt e.V. VELUX Group
Hegelplatz 1 Ådalsvej 99
10117 Berlin 2970 Hørsholm
Germany Denmark
Declaration number Declared product / declared unit
EPD-VEL-20220111-CBB3-EN 1m² underfelt collar BFX
The declared unit is based on the configuration of a standard size window
measuring 0.78m x 1.178m.
This declaration is based on the product category rules: Scope:
Windows and doors , 01.08.2021 Productline BFX - Collar/installation product; manufactured by VELUX in
(PCR checked and approved by the SVR) France for sale in Europe.
Declaration according to ISO 14025 and EN 15804 describing specific
Issue date environmental performances of the construction product.
The owner of the declaration shall be liable for the underlying information
24.05.2022
and evidence; the IBU shall not be liable with respect to manufacturer
information, life cycle assessment data and evidences.
Valid to
The EPD was created according to the specifications of EN 15804+A2. In
23.05.2027 the following, the standard will be simplified as EN 15804.
Verification
The standard EN 15804 serves as the core PCR
Independent verification of the declaration and data according to ISO
14025:2011
internally X externally
Dipl.-Ing. Hans Peters
(Chairman of Institut Bauen und Umwelt e.V.)
Florian Pronold Prof. Dr. Birgit Grahl,
(Managing Director Institut Bauen und Umwelt e.V.) (Independent verifier)
1 Environmental Product Declaration - Velux - Collar BFX
Product
Performance data of the product in accordance with the
Product description/Product definition declaration of performance with respect to its essential
The VELUX BFX underfelt collar is a product for sale in the characteristics according to DIN EN 13859-1:2014 - Flexible
European market. sheets for waterproofing – Definitions and characteristics of
underlays – Part 1:
The underfelt collar consists of mainly steel and plastics. Underlays for discontinuous roofing.
The calculations are based on the BFX underfelt collar. For the Base materials/Ancillary materials
placing on the market of the product in the European Name Value Unit
Union/European Free Trade Association (EU/EFTA) (with the
Galvanized steel 67 %
exception of Switzerland) Regulation (EU) No. 305/2011 (CPR)
Polypropylene 16 %
applies. The product needs a declaration of performance taking
Polybutadiene 16 %
into consideration DIN EN 13859-1:2014 - Flexible sheets for
waterproofing - Definitions and characteristics of underlays - Hot-melt adhesive 0.3 %
Part 1: Underlays for discontinuous roofing. For the application
REACH
and use the respective national provisions apply.
This product/article/at least one partial article contains
Application
substances listed in the candidate list (date: 17.01.2022)
VELUX BFX underfelt collar is used in renovation and new
exceeding 0.1 percentage by mass: no.
build.
Technical Data Recycled content
The Declaration of Performance including relevant technical
specifications and test methods/test standards can be
downloaded from the website www.velux.com/ce-marking.
The performance values are specific for the BFX underfelt
The values stated in the table relate to the recycled material
collar.
streams in VELUX production.
The declared values in the table relate to the reference product.
For other covered product variants, specific values can be Reference service life
selected at the bottom of the above-mentioned download page.
A calculation of the reference service life according to ISO
15686 is not possible.
Constructional data
The Bundesinstitut für Bau, Stadt und Raumforschung/Federal
Name Value Unit
office for building and regional planning (BBSR)
Fire resistance class DIN EN 1634-1 E class
table declares for the complete roof window a service life
Resistance to water penetration before class
dependent on the applied window frame material between 25
artificial ageing W1
and ≥ 50 years. This includes collars and flashings as declared
Resistance to water penetration after artificial class with this EPD.
ageing W1
Tensile strength in longitudinal direction
200 N/50mm
before artificial ageing
Tensile strength in longitudinal direction after
120 N/50mm
artificial ageing
Tensile strength in transverse direction
200 N/50mm
before artificial ageing
Tensile strength in transverse direction after
120 N/50mm
artificial ageing
LCA: Calculation rules
Declared Unit
The declared unit is one m² related to a reference window, that System boundary
the collar is installed in connection with. Type of EPD: Cradle to gate - with options. The following life
cycle stages were considered:
The declared unit is based on the representative product
measuring 0.78m x 1.178m. Production stage A1-A3:
Consideration of the production of raw materials and their
Declared unit
processing; transport of major material to the manufacturing
Name Value Unit
site; assembly of semi-finished products to the final product;
Declared unit 1 m2 packaging material (including waste paper input for paper and
Weight per area 1.77 kg/representative product cardboard).
Weight per area 1.92 kg/declared unit
End-of-Life stage C1, C2, C3:
2 Environmental Product Declaration - Velux - Collar BFX
declared in module D.
C1: a manual demolition is assumed, resulting in indicator value
"0". Contribution of waste flows is considered in the modules where
C2: For the transport to EoL by truck a distance of 50 km is they occur.
assumed.
C3: A scenario for the incineration of plastics in a waste Geographic Representativeness
incineration plant (WIP) is assumed. Land or region, in which the declared product system is
manufactured, used or handled at the end of the product´s
The EoL-Scenario does not assume waste to be disposed of on lifespan: Europe
a landfill site. Module C4 is declared as "0".
Comparability
Benefits for the next product system D:
Basically, a comparison or an evaluation of EPD data is only
possible if all the data sets to be compared were created
Resulting electrical and thermal energy from the WIP, avoiding
according to EN 15804 and the building context, respectively
the generation of electricity and heat via fossil fuels, is
the product-specific characteristics of performance, are taken
considered.
into account. The software GaBi is used accompanied by the
The amount of metals after the reduction due to the net-flow
GaBi background data base (version 2021.2, 2021).
calculations is sent to a recycling process. The effort for
recycling, as well as the benefit for the regained metals are
LCA: Scenarios and additional technical information
Characteristic product properties of biogenic carbon
The following declared values refer to the declared unit of 1m².
Information on describing the biogenic Carbon Content at
factory gate Reference service life
The declared biogenic content comprises the paper manual Name Value Unit
and the packaging material consisting of cardboard, paper and
Life Span (according to BBSR) depending on 25 -
wood. As module A5 is not declared, the information on a
window frame material 50
packaging supports further EoL calculations.
Name ValueUnit End of life (C1-C4)
kg Name Value Unit
Biogenic carbon content in product -
C Collected separately waste type waste type 1.92 kg
Biogenic carbon content in accompanying 0.147 kg Recycling 1.29 kg
packaging C
Energy recovery 0.62 kg
The value refers to the following packaging material (per 1m²):
Paper (manual): 0.009kg, Cardboard packaging: 0.329kg, Reuse, recovery and/or recycling potentials (D), relevant
Paper insert: 0.003kg, PE-LD: 0.009kg scenario information
Name Value Unit
Note: 1 kg of biogenic carbon is equivalent to 44/12 kg of CO .
2 Steel (net-flow calculation) 1.63 kg/1m² product
3 Environmental Product Declaration - Velux - Collar BFX
LCA: Results
DESCRIPTION OF THE SYSTEM BOUNDARY (X = INCLUDED IN LCA; MND = MODULE OR INDICATOR NOT DECLARED; MNR
= MODULE NOT RELEVANT)
Benefits and
Construction loads beyond
Product stage Use stage End of life stage
process stage the system
boundaries
la ire ta m w a Ry lp p u s tro p s n a rT g n iru tc a fu n a M e h t m o rf tro p s n a rTe tis e h t o t e ta g y lb m e s s A e s U e c n a n e tn ia M ria p e R tn e m e c a lp e R tn e m h s ib ru fe R y g re n e la n o ita re p Oe s u re ta w la n o ita re p Oe s u n o itc u rts n o c -e Dn o itilo m e d tro p s n a rT g n is s e c o rp e ts a W la s o p s iD -e s u e R-y re v o c e R-g n ilc y c e Rla itn e to p
A1 A2 A3 A4 A5 B1 B2 B3 B4 B5 B6 B7 C1 C2 C3 C4 D
X X X MND MND MND MND MNR MNR MNR MND MND X X X X X
RESULTS OF THE LCA - ENVIRONMENTAL IMPACT according to EN 15804+A2: 1 m² BFX
Parameter Unit A1-A3 C1 C2 C3 C4 D
Global Warming Potential total (GWP-total) kg CO 2 eq 6.69E+00 0 5.84E-03 2.39E+00 0 -3.41E+00
Global Warming Potential fossil fuels (GWP-fossil) kg CO 2 eq 7.2E+00 0 5.8E-03 2.39E+00 0 -3.4E+00
Global Warming Potential biogenic (GWP-biogenic) kg CO 2 eq -5.15E-01 0 -6.9E-06 1.26E-04 0 -7.17E-03
Global Warming Potential luluc (GWP-luluc) kg CO 2 eq 3.39E-03 0 4.73E-05 6.48E-05 0 -8.66E-04
Depletion potential of the stratospheric ozone layer (ODP) kg CFC11 eq 5.3E-12 0 1.14E-18 5.47E-16 0 -1.88E-14
Acidification potential of land and water (AP) mol H+ eq 1.8E-02 0 1.14E-05 2.79E-04 0 -5.5E-03
Eutrophication potential aquatic freshwater (EP-freshwater) kg P eq 3.4E-05 0 1.72E-08 8.34E-08 0 -2.03E-06
Eutrophication potential aquatic marine (EP-marine) kg N eq 4.36E-03 0 4.74E-06 7.15E-05 0 -1.2E-03
Eutrophication potential terrestrial (EP-terrestrial) mol N eq 4.58E-02 0 5.37E-05 1.28E-03 0 -1.24E-02
Formation potential of tropospheric ozone photochemical oxidants kg NMVOC
1.91E-02 0 1.02E-05 2.08E-04 0 -4.65E-03
(POCP) eq
Abiotic depletion potential for non fossil resources (ADPE) kg Sb eq 2.38E-05 0 5.13E-10 7.96E-09 0 -5.72E-06
Abiotic depletion potential for fossil resources (ADPF) MJ 1.24E+02 0 7.72E-02 7.15E-01 0 -4.22E+01
m3 world eq
Water use (WDP) 3.41E+00 0 5.38E-05 2.35E-01 0 -6.16E+00
deprived
RESULTS OF THE LCA - INDICATORS TO DESCRIBE RESOURCE USE according to EN 15804+A2: 1 m² BFX
Parameter Unit A1-A3 C1 C2 C3 C4 D
Renewable primary energy as energy carrier (PERE) MJ 4.11E+00 0 4.44E-03 1.53E-01 0 -3.27E+00
Renewable primary energy resources as material utilization
MJ 5.43E+00 0 0 0 0 0
(PERM)
Total use of renewable primary energy resources (PERT) MJ 9.54E+00 0 4.44E-03 1.53E-01 0 -3.27E+00
Non renewable primary energy as energy carrier (PENRE) MJ 9.66E+01 0 7.74E-02 2.84E+01 0 -4.22E+01
Non renewable primary energy as material utilization (PENRM) MJ 2.77E+01 0 0 -2.77E+01 0 0
Total use of non renewable primary energy resources (PENRT) MJ 1.24E+02 0 7.74E-02 7.15E-01 0 -4.22E+01
Use of secondary material (SM) kg 3.98E-01 0 0 0 0 1.31E+00
Use of renewable secondary fuels (RSF) MJ 0 0 0 0 0 0
Use of non renewable secondary fuels (NRSF) MJ 0 0 0 0 0 0
Use of net fresh water (FW) m3 9.2E-02 0 5.09E-06 5.55E-03 0 -1.46E-01
RESULTS OF THE LCA – WASTE CATEGORIES AND OUTPUT FLOWS according to EN 15804+A2:
1 m² BFX
Parameter Unit A1-A3 C1 C2 C3 C4 D
Hazardous waste disposed (HWD) kg 1.42E-07 0 4.08E-12 1.28E-10 0 1.66E-10
Non hazardous waste disposed (NHWD) kg 2.13E-01 0 1.21E-05 1.57E-01 0 2.68E-01
Radioactive waste disposed (RWD) kg 4.71E-03 0 1.4E-07 2.95E-05 0 -1.49E-03
Components for re-use (CRU) kg 0 0 0 0 0 0
Materials for recycling (MFR) kg 0 0 0 1.04E+00 0 0
Materials for energy recovery (MER) kg 0 0 0 0 0 0
Exported electrical energy (EEE) MJ 0 0 0 5.09E+00 0 0
Exported thermal energy (EET) MJ 0 0 0 9.14E+00 0 0
RESULTS OF THE LCA – additional impact categories according to EN 15804+A2-optional:
1 m² BFX
Parameter Unit A1-A3 C1 C2 C3 C4 D
Disease
Incidence of disease due to PM emissions (PM) 1.98E-07 0 6.94E-11 3.32E-09 0 -8.86E-08
incidence
Human exposure efficiency relative to U235 (IR) kBq U235 eq 1.18E+00 0 2.05E-05 4.02E-03 0 -2.04E-01
Comparative toxic unit for ecosystems (ETP-fw) CTUe 7.62E+01 0 5.73E-02 4.86E-01 0 -5.7E+00
Comparative toxic unit for humans (carcinogenic) (HTP-c) CTUh 2.9E-09 0 1.16E-12 2.89E-11 0 -1.4E-09
4 Environmental Product Declaration - Velux - Collar BFX
Comparative toxic unit for humans (noncarcinogenic) (HTP-nc) CTUh 9.62E-08 0 6.29E-11 2.75E-09 0 -3.45E-08
Soil quality index (SQP) SQP 2.4E+01 0 2.65E-02 1.77E-01 0 -2.85E+00
Disclaimer 1 – for the indicator 'Potential Human exposure efficiency relative to U235'.
This impact category deals mainly with the eventual impact of low dose ionizing radiation on human health of the nuclear fuel cycle. It
does not consider effects due to possible nuclear accidents, occupational exposure or radioactive waste disposal in underground
facilities. Potential ionizing radiation from the soil, radon and from some construction materials is also not measured by this indicator.
Disclaimer 2 – for the indicators 'abiotic depletion potential for non-fossil resources', 'abiotic depletion potential for fossil resources',
'water (user) deprivation potential, deprivation-weighted water consumption', 'potential comparative toxic unit for ecosystems', 'potential
comparative toxic unit for humans – cancerogenic', 'Potential comparative toxic unit for humans - not cancerogenic', 'potential soil
quality index'. The results of this environmental impact indicator shall be used with care as the uncertainties on these results are high
or as there is limited experience with the indicator.
Disclaimer 3 – for 'potential soil quality index'. Due to a data lack in the foreground data of VELUX, the result has a very high
uncertainty and refers only to the background data, which contain respective information.
References
BBSR EN ISO 14025:2011, Environmental labels and declarations —
BBSR, 24.02.2017, Nutzungsdauer von Bauteilen nach BNB Type III environmental declarations — Principles and
procedures.
DIN EN 1634-1
DIN EN 1634-1:2018-04: Fire resistance and smoke control ISO 15686
tests for door and shutter assemblies, openable windows and ISO 15686:2011-05: Buildings and constructed assets - Service
elements of building hardware - Part 1: Fire resistance test for life planning - Part 1: General principles and framework
door and shutter assemblies and openable windows
PCR part A
DIN EN 13859-1 Calculation Rules for the Life Cycle Assessment and
DIN EN 13859-1:2014-07: Flexible sheets for waterproofing - Requirements on the Project Report according to EN
Definitions and characteristics of underlays - Part 1: Underlays 15804+A2:2019, version 1.2, Berlin: Institut Bauen und Umwelt
for discontinuous roofing e.V., 2021
EN 15804 PCR part B
EN 15804:2012+A2:2019, Sustainability of construction works Requirements on the EPDS for Windows and doors, version
— Environmental Product Declarations — Core rules for the 01-2021, Berlin: Institut Bauen und Umwelt e.V.
product category of construction products.
REACH
GaBi Regulation (EC) No 1907/2006 of the European Parliament and
GaBi Software and GaBi Database by Sphera Solution GmbH, of the Council on the Registration, Evaluation, Authorisation
version: 2021.2, 2021 and Restriction of Chemicals (REACH)
IBU 2021 Regulation (EU) No. 305/2011 (CPR)
Institut Bauen und Umwelt e.V.: General Instructions for the Regulation (EU) No 305/2011 of the European Parliament and
EPD programme of Institut Bauen und Umwelt e.V., Version of the Council of 9 March 2011 laying down harmonized
2.0, Berlin: Institut Bauen und Umwelt e.V., 2021, www.ibu- conditions for the marketing of construction products and
epd.com repealingCounsicl Directive 89/106/EEC
ISO 14025
5 Environmental Product Declaration - Velux - Collar BFX
Publisher
Institut Bauen und Umwelt e.V. +49 (0)30 3087748- 0
Hegelplatz 1 info@ibu-epd.com
10117 Berlin www.ibu-epd.com
Germany
Programme holder
Institut Bauen und Umwelt e.V. +49 (0)30 3087748- 0
Hegelplatz 1 info@ibu-epd.com
10117 Berlin www.ibu-epd.com
Germany
Author of the Life Cycle Assessment
Angela Schindler Umweltberatung 07553 919 9456
Tüfinger Str. 12 angela@schindler-umwelt.de
88682 Salem www.schindler-umwelt.de
Germany
Daxner & Merl GmbH +43 676 849477826
Lindengasse 39/8 office@daxner-merl.com
1070 Wien www.daxner-merl.com
Austria
Owner of the Declaration
VELUX Group +4545164726
Ådalsvej 99 jakob.roerbech@velux.com
2970 Hørsholm www.velux.com
Denmark
6 Environmental Product Declaration - Velux - Collar BFX
