ENVIRONMENTAL PRODUCT DECLARATION
as per ISO 14025 and EN 15804+A2
Owner of the Declaration VELUX Group
Publisher Institut Bauen und Umwelt e.V. (IBU)
Programme holder Institut Bauen und Umwelt e.V. (IBU)
Declaration number EPD-VEL-20230048-IBA2-EN
Issue date 11.05.2023
Valid to 10.05.2028
Window operator for VELUX pivot hinged windows mains
connected
VELUX Group
www.ibu-epd.com | https://epd-online.com
General Information
VELUX Group Window operator for VELUX pivot hinged windows
mains connected
Programme holder Owner of the declaration
IBU – Institut Bauen und Umwelt e.V. VELUX Group
Hegelplatz 1 Ådalsvej 99
10117 Berlin 2970 Hørsholm
Germany Denmark
Declaration number Declared product / declared unit
EPD-VEL-20230048-IBA2-EN The declared unit is one piece of electrical window operator.
This declaration is based on the product category rules: Scope:
Drive systems for automatic doors and gates, 01.08.2021 The EPD is a specific EPD covering VELUX electrical window operator for
(PCR checked and approved by the SVR) the mains connected pivot hinged windows. The operator consists of a
chain operator, a rain sensor, a power supply and a remote. The products
are manufactured by the VELUX Group at a production site in the Czech
Issue date Republic.
The owner of the declaration shall be liable for the underlying information
11.05.2023
and evidence; the IBU shall not be liable with respect to manufacturer
information, life cycle assessment data and evidences.
Valid to
The EPD was created according to the specifications of EN 15804+A2. In
10.05.2028 the following, the standard will be simplified as EN 15804.
Verification
The standard EN 15804 serves as the core PCR
Independent verification of the declaration and data according to ISO
14025:2011
internally X externally
Dipl.-Ing. Hans Peters
(Chairman of Institut Bauen und Umwelt e.V.)
Florian Pronold Dr.-Ing. Nikolay Minkov,
(Managing Director Institut Bauen und Umwelt e.V.) (Independent verifier)
1 Environmental Product Declaration - VELUX Group - Window operator for VELUX pivot hinged windows mains connected
Product
Product description/Product definition
EPD covering VELUX electrical window operator for the mains Base materials/Ancillary materials
connected pivot hinged windows. The operator consists of a
Product content
chain operator, a rain sensor, a power supply and a remote.
Name Value Unit
The products are manufactured by the VELUX Group at a
production site in the Czech Republic. For the placing on the Other plastic components 34 %
market of the product in the European Union/European Free Cables 26 %
Trade Association (EU/EFTA) (with the exception of Other metal components 19 %
Switzerland) Regulation (EU) No. 305/2011 (CPR) applies. The
PCBA 7 %
products are in compliance with the Machinery Directive
Motor 5 %
2006/42/EC, the Radio Equipment Directive 2014/53/EU and
the RoHS Directive 2011/65/EU. A declaration of conformity is Battery 2 %
available from the manufacturer. Other (butyl sealant, epoxy, paper) 8 %
This product/article/at least one partial article contains
Application
substances listed in the candidate list (date: 08.06.2022)
The VELUX electrical window operator is installed in new
exceeding 0.1 percentage by mass: NO.
windows before distribution to customers.
Reference service life
Technical Data
No reference service life (RSL) is defined for the operators as
The CE marking for electrical window operators does not
the use stage modules are not included in the EPD. There is no
specify the need for a Declaration of Performance. Instead, a
generally acknowledged or common way to assess the RSL for
Declaration of Conformity is required.
this type of product. Furthermore, the lifetime of the products
The performance values relevant for the product are specified
depends greatly on the use pattern and environmental
in the table below.
conditions in use, which differs for different users and which is
Constructional data difficult to predict at the time of sale.
Name Value Unit
Protection class IP 44 class
Voltage 230 V
LCA: Calculation rules
A3 - Manufacturing: The products are produced/assembled at
Declared Unit the VELUX production site, where the finished window operator
The declared unit is one piece. This corresponds to an is ready for shipment.
electrical window operator system, including a chain operator, a
power supply, a rain sensor and a remote. End of life stage:
Name Value Unit
Declared unit 1 pce. C1 - De-construction/demolition: de-construction of the product
with the use of manual hand tools.
Weight 1,6 kg
Conversion factor to kg 0,625
C2 - Transport: transport of the product to waste treatment
Other declared units are allowed if the conversion is shown including to and from sorting and shredding facilities.
transparently.
C3 - Waste processing: includes sorting, shredding, incineration
A data quality and a sensitivity analysis show that the results and recycling processes.
are robust with regard to data quality and appropriateness.
There is low variability of production processes and product C4 - Disposal: disposal of all materials
variations have a limited influence on the results.
Benefits and loads beyond the system boundaries:
System boundary
Type of EPD: D - Reuse, recovery and recycling potential: benefits from
plastic incineration processes and material recycling. End-of-life
Cradle to gate - with options. The following life cycle phases includes all activities from when the product reaches the end of
were considered: its service life and no longer provides any functionality until all
Product stage: materials and components are processed for
reuse/recycling/energy recovery or are disposed of.
A1 - Raw material supply: extraction and processing,
production of the pre-products (e.g. motor suspension, PCB, The applied end-of-life scenario follows the requirements in the
battery...). Sales packaging is not included, since the products PCR Part A, chapter 6.2 regarding complex products, with a
are integrated with the window. VELUX roof window EPD's combination of recycling, thermal waste treatment and
include the packaging. landfilling. 100% of the material is considered in the end-of-life
scenario. Generally metals, cables, batteries and
A2 - Transport: Transport of pre-products and packaging polychlorinated biphenyl (PCB)'s are recycled, plastic parts are
components to the manufacturing sites incinerated with energy recovery and magnets are landfilled.
2 Environmental Product Declaration - VELUX Group - Window operator for VELUX pivot hinged windows mains connected
Basically, a comparison or an evaluation of EPD data is only
Geographic Representativeness possible if all the data sets to be compared were created
Land or region, in which the declared product system is according to EN 15804 and the building context, respectively
manufactured, used or handled at the end of the product´s the product-specific characteristics of performance, are taken
lifespan: Europe into account. The used background software and database is
GaBi (DB version 2021.2)
Comparability
LCA: Scenarios and additional technical information
End of life (C1-C4)
Characteristic product properties of biogenic carbon
The product does not contain biogenic carbon. Name Value Unit
Collected separately waste type Electronics 1.6 kg
Information on describing the biogenic Carbon Content at
factory gate Recycling 0.91 kg
Name ValueUnit Energy recovery 0.67 kg
kg Landfilling 0.03 kg
Biogenic carbon content in product -
C
Reuse, recovery and/or recycling potentials (D), relevant
Biogenic carbon content in accompanying kg
- scenario information
packaging C
Name Value Unit
Replaced materials 0.17 kg
Replaced thermal energy 3.4 MJ
No Reference Service Life (RFL) is declared, because the use Replaced electricity 1.9 MJ
stage modules are not declared.
3 Environmental Product Declaration - VELUX Group - Window operator for VELUX pivot hinged windows mains connected
LCA: Results
DESCRIPTION OF THE SYSTEM BOUNDARY (X = INCLUDED IN LCA; MND = MODULE OR INDICATOR NOT DECLARED; MNR
= MODULE NOT RELEVANT)
Benefits and
Construction loads beyond
Product stage Use stage End of life stage
process stage the system
boundaries
la ire ta m w a Ry lp p u s tro p s n a rT g n iru tc a fu n a M e h t m o rf tro p s n a rTe tis e h t o t e ta g y lb m e s s A e s U e c n a n e tn ia M ria p e R tn e m e c a lp e R tn e m h s ib ru fe R y g re n e la n o ita re p Oe s u re ta w la n o ita re p Oe s u n o itc u rts n o c -e Dn o itilo m e d tro p s n a rT g n is s e c o rp e ts a W la s o p s iD -e s u e R-y re v o c e R-g n ilc y c e Rla itn e to p
A1 A2 A3 A4 A5 B1 B2 B3 B4 B5 B6 B7 C1 C2 C3 C4 D
X X X MND MND MND MND MNR MNR MNR MND MND X X X X X
RESULTS OF THE LCA - ENVIRONMENTAL IMPACT according to EN 15804+A2: 1 pcs window operator
Parameter Unit A1 A2 A3 C1 C2 C3 C4 D
GWP-total kg CO 2 eq 1.06E+01 4.16E-01 7.86E-01 0 8.53E-03 1.43E+00 1.47E-05 -1.18E+00
GWP-fossil kg CO 2 eq 1.07E+01 4.14E-01 5.98E-01 0 8.47E-03 1.43E+00 1.51E-05 -1.18E+00
GWP-biogenic kg CO 2 eq -1.33E-01 1.82E-04 1.88E-01 0 -1.08E-05 1.24E-03 -4.39E-07 3.13E-04
GWP-luluc kg CO 2 eq 1.57E-02 1.13E-03 4.5E-05 0 6.93E-05 1.67E-04 4.44E-08 -1.43E-03
ODP kg CFC11 eq 1.3E-09 4.6E-17 2.93E-15 0 1.08E-18 6.66E-09 5.88E-20 -6.18E-15
AP mol H+ eq 4.9E-02 1.06E-02 1.01E-03 0 2.65E-05 1.7E-03 1.08E-07 -3.96E-03
EP-freshwater kg P eq 1.52E-04 4.7E-07 1.79E-06 0 2.51E-08 1.09E-05 2.54E-11 -1.13E-06
EP-marine kg N eq 8.14E-03 2.89E-03 2.14E-04 0 1.22E-05 7.79E-04 2.8E-08 -6.47E-04
EP-terrestrial mol N eq 8.6E-02 3.17E-02 2.28E-03 0 1.36E-04 8.56E-03 3.07E-07 -6.98E-03
kg NMVOC
POCP 2.59E-02 7.9E-03 5.98E-04 0 2.38E-05 2E-03 8.47E-08 -1.94E-03
eq
ADPE kg Sb eq 8.93E-04 1.87E-08 4E-08 0 6.45E-10 2.19E-07 1.43E-12 -4.03E-05
ADPF MJ 1.62E+02 5.18E+00 8.79E+00 0 1.13E-01 2.3E+00 2.01E-04 -1.6E+01
m3 world eq
WDP 4.63E+00 1.62E-03 2.98E-02 0 7.35E-05 4.96E-01 1.62E-06 -2.57E-01
deprived
GWP = Global warming potential; ODP = Depletion potential of the stratospheric ozone layer; AP = Acidification potential of land and water; EP =
Eutrophication potential; POCP = Formation potential of tropospheric ozone photochemical oxidants; ADPE = Abiotic depletion potential for non-fossil
resources; ADPF = Abiotic depletion potential for fossil resources; WDP = Water (user) deprivation potential)
RESULTS OF THE LCA - INDICATORS TO DESCRIBE RESOURCE USE according to EN 15804+A2: 1 pcs window operator
Parameter Unit A1 A2 A3 C1 C2 C3 C4 D
PERE MJ 2.83E+01 1.14E-01 4.2E-01 0 6.29E-03 7.14E-01 2.7E-05 -3.38E+00
PERM MJ 0 0 0 0 0 0 0 0
PERT MJ 2.83E+01 1.14E-01 4.2E-01 0 6.29E-03 7.14E-01 2.7E-05 -3.38E+00
PENRE MJ 1.44E+02 5.19E+00 8.79E+00 0 1.13E-01 1.5E+01 2.01E-04 -1.6E+01
PENRM MJ 1.81E+01 0 0 0 0 -1.27E+01 0 0
PENRT MJ 1.62E+02 5.19E+00 8.79E+00 0 1.13E-01 2.3E+00 2.01E-04 -1.6E+01
SM kg 1.78E-01 0 0 0 0 0 0 0
RSF MJ 0 0 0 0 0 0 0 0
NRSF MJ 0 0 0 0 0 0 0 0
FW m3 1.23E-01 1.36E-04 2.41E-03 0 7.2E-06 1.19E-02 4.95E-08 -1.06E-02
PERE = Use of renewable primary energy excluding renewable primary energy resources used as raw materials; PERM = Use of renewable primary
energy resources used as raw materials; PERT = Total use of renewable primary energy resources; PENRE = Use of non-renewable primary energy
excluding non-renewable primary energy resources used as raw materials; PENRM = Use of non-renewable primary energy resources used as raw
materials; PENRT = Total use of non-renewable primary energy resources; SM = Use of secondary material; RSF = Use of renewable secondary fuels;
NRSF = Use of non-renewable secondary fuels; FW = Use of net fresh water
RESULTS OF THE LCA – WASTE CATEGORIES AND OUTPUT FLOWS according to EN 15804+A2:
1 pcs window operator
Parameter Unit A1 A2 A3 C1 C2 C3 C4 D
HWD kg 1.09E-04 1.18E-10 1.39E-09 0 5.69E-12 5E-10 2.13E-14 -2.3E-09
NHWD kg 6.19E-01 6.09E-04 9.73E-03 0 1.68E-05 1.15E-01 1E-03 -5E-02
RWD kg 2.99E-03 5.95E-06 9.99E-04 0 1.37E-07 2.09E-04 2.11E-09 -6.86E-04
CRU kg 0 0 0 0 0 0 0 0
MFR kg 0 0 0 0 0 7.15E-01 0 0
MER kg 0 0 0 0 0 5.48E-01 0 0
EEE MJ 0 0 0 0 0 0 0 1.88E+00
EET MJ 0 0 0 0 0 0 0 3.4E+00
4 Environmental Product Declaration - VELUX Group - Window operator for VELUX pivot hinged windows mains connected
HWD = Hazardous waste disposed; NHWD = Non-hazardous waste disposed; RWD = Radioactive waste disposed; CRU = Components for re-use;
MFR = Materials for recycling; MER = Materials for energy recovery; EEE = Exported electrical energy; EET = Exported thermal energy
RESULTS OF THE LCA – additional impact categories according to EN 15804+A2-optional:
1 pcs window operator
Parameter Unit A1 A2 A3 C1 C2 C3 C4 D
Disease
PM 6.05E+01 3.65E+00 8.32E-01 0 7.92E-02 1.07E+01 1.07E-04 -3.96E+00
incidence
IR kBq U235 eq 3.03E+01 6.41E-02 1.6E+00 0 1.53E-03 1.49E+00 6.15E-06 -1.61E+00
ETP-fw CTUe 3.84E-01 3.31E-02 2.1E-03 0 7.61E-04 4.92E-02 8.69E-07 -4.09E-02
HTP-c CTUh 2.91E-19 1.23E-21 1.35E-21 0 2.83E-23 5.41E-20 1.85E-25 -1.96E-19
HTP-nc CTUh 3.69E-09 7.02E-11 3.61E-11 0 1.61E-12 7.88E-10 1.64E-14 -8.84E-10
SQP SQP 7.44E-08 1.58E-12 2.35E-11 0 3.76E-14 2.54E-11 4.93E-16 -3.56E-10
PM = Potential incidence of disease due to PM emissions; IR = Potential Human exposure efficiency relative to U235; ETP-fw = Potential comparative
Toxic Unit for ecosystems; HTP-c = Potential comparative Toxic Unit for humans (cancerogenic); HTP-nc = Potential comparative Toxic Unit for humans
(not cancerogenic); SQP = Potential soil quality index
Disclaimer 1 – for the indicator “Potential Human exposure efficiency relative to U235”. This impact category deals mainly with the
eventual impact of low-dose ionizing radiation on human health of the nuclear fuel cycle. It does not consider effects due to possible
nuclear accidents, occupational exposure or radioactive waste disposal in underground facilities. Potential ionizing radiation from the
soil, radon and from some construction materials is also not measured by this indicator.
Disclaimer 2 – for the indicators “abiotic depletion potential for non-fossil resources”, “abiotic depletion potential for fossil resources”,
“water (user) deprivation potential, deprivation-weighted water consumption”, “potential comparative toxic unit for ecosystems”,
“potential comparative toxic unit for humans – cancerogenic”, “Potential comparative toxic unit for humans - not cancerogenic”,
“potential soil quality index”. The results of this environmental impact indicator shall be used with care as the uncertainties on these
results are high as there is limited experience with the indicator.
References
IBU PCR Part A Directive 2006/42/EC of the European Parliament and of the
IBU PCR Part A: Institut Bauen und Umwelt e.V., Product Council, 17 May 2006 on Machinery
Category Rules for Building-Related Products and Services.
Calculation Rules for the Life Cycle Assessment and EN 14351-1:2006+A2:2016
Requirements on the Project Report according to EN EN14351-1:2006+A2:2016, Windows and doors - Product
15804+A2:2019. standard, performance characteristics - Part 1: Windows and
external pedestrian doorsets.
IBU PCR Part B
IBU PCR Part B: Institut Bauen und Umwelt e.V., Requirements EN 15804:2019+A2
on the EPD for Drive systems for automatic doors and gates, EN15804:2019+A2: Sustainability of construction works -
version 1.6. Environmental Product Declarations - Core rules for the product
category of construction products.
IBU 2021
IBU 2021: Institut Bauen und Umwelt e.V.: General Instructions Directive 2014/53/EU
for the EPD programme of Institut Bauen und Umwelt e.V. Directive 2014/53/EU of the European Parliament and of the
Version 2.0, Berlin: Institut Bauen und Umwelt e.V., 2021. Council of 16 April 2014 on the harmonisation of the laws of the
www.ibu-epd.com. Member States relating to the making available on the market
of radio equipment
EN 13501-1:2018
EN13501-1, 2018: Fire classification of construction products Directive 2011/65/EU
and building elements - Part 1: Classification using data from Directive 2011/65/EU of the European Parliament and of the
reaction to fire tests. Council of 8 June 2011 on the restriction of the use of certain
hazardous substances in electrical and electronic equipment
DIN EN ISO 14025:2011-10
DIN EN ISO14025:2011-10, Environmental labels and Directive 2006/42/EC
declarations - Type III environmental declarations - Principles DIRECTIVE 2006/42/EC OF THE EUROPEAN PARLIAMENT
and procedures. AND OF THE COUNCIL of 17 May 2006 on machinery
Regulation (EU) No 305/2011 Candidate list
Regulation (EU) No 305/2011 of the European Parliament and Candidate List of substances of very high concern for
of the Council, 9 March 2011, Laying down harmonised Authorisation, 08.06.2022.
conditions for the marketing of constructional products.
GaBi LCA software and database
Directive 2011/65/EU The LCA modelling software is GaBi program version
Directive 2011/65/EU of the European Parliament and of the 10.5.1.124 with corresponding databases from Sphera
Council, 8 June 2011, on the restriction of the use of certain Solutions GmbH. Documentation hyperlink www.gabi-
hazardous substances in electrical and electronic equipment. software.com/support/gabi.
Directive 2006/42/EC
5 Environmental Product Declaration - VELUX Group - Window operator for VELUX pivot hinged windows mains connected
Publisher
Institut Bauen und Umwelt e.V. +49 (0)30 3087748- 0
Hegelplatz 1 info@ibu-epd.com
10117 Berlin www.ibu-epd.com
Germany
Programme holder
Institut Bauen und Umwelt e.V. +49 (0)30 3087748- 0
Hegelplatz 1 info@ibu-epd.com
10117 Berlin www.ibu-epd.com
Germany
Author of the Life Cycle Assessment
FORCE Technology +4543250856
Park Alle 345 chme@force.dk
2605 Brøndby www.forcetechnology.com
Denmark
Owner of the Declaration
VELUX Group +4545164726
Ådalsvej 99 jakob.roerbech@velux.com
2970 Hørsholm www.velux.com
Denmark
6 Environmental Product Declaration - VELUX Group - Window operator for VELUX pivot hinged windows mains connected
