ENVIRONMENTAL PRODUCT DECLARATION
as per ISO 14025 and EN 15804+A2
Owner of the Declaration VELUX Group
Publisher Institut Bauen und Umwelt e.V. (IBU)
Programme holder Institut Bauen und Umwelt e.V. (IBU)
Declaration number EPD-VEL-20230507-CBA1-EN
Issue date 11/03/2024
Valid to 10/03/2029
VELUX lining LSB
VELUX A/S
www.ibu-epd.com | https://epd-online.com
General Information
VELUX A/S VELUX lining LSB
Programme holder Owner of the declaration
IBU – Institut Bauen und Umwelt e.V. VELUX Group
Hegelplatz 1 Ådalsvej 99
10117 Berlin 2970 Hørsholm
Germany Denmark
Declaration number Declared product / declared unit
EPD-VEL-20230507-CBA1-EN 1m² lining LSB.
The declared unit is based on the configuration of a standard size window
measuring 0.78 m x 1.178 m.
The product LSB is manufactured in Germany.
(The declared representative product of the product group comprise the
product with the highest mass.)
This declaration is based on the product category rules: Scope:
Windows and doors , 01/08/2021 Productline LSB - lining; manufactured by VELUX in Germany for sale in
(PCR checked and approved by the SVR) Europe.
Declaration according to ISO 14025 and EN 15804 describing specific
Issue date environmental performance of the construction product.
The owner of the declaration shall be liable for the underlying information
11/03/2024
and evidence; the IBU shall not be liable with respect to manufacturer
information, life cycle assessment data and evidences.
Valid to
The EPD was created according to the specifications of EN 15804+A2. In
10/03/2029 the following, the standard will be simplified as EN 15804.
Verification
The standard EN 15804 serves as the core PCR
Independent verification of the declaration and data according to ISO
14025:2011
internally X externally
Dipl.-Ing. Hans Peters
(Chairman of Institut Bauen und Umwelt e.V.)
Florian Pronold Dr.-Ing. Nikolay Minkov,
(Managing Director Institut Bauen und Umwelt e.V.) (Independent verifier)
1 Environmental Product Declaration - VELUX A/S - VELUX lining LSB
Product
Product description/Product definition Technical Data
VELUX linings ensure an easy and quick connection of the roof The Declaration of Performance including relevant technical
window to the interior ceiling finish. They and their facings are specifications and test methods/test standards can be
assembled before being clicked into the window rebate in one downloaded from the website www.velux.com/ce-marking.
piece from the inside and there is no need for further framing.
Constructional data
Name Value Unit
The linings are made in white PVC, need no finishing treatment Reaction to fire E class
and are not sensitive to moisture. The white, semi-gloss surface Durability No performance determined
and the white facings supplied ensure a harmonious connection
Performance data of the product in accordance with the
from the roof window to most walls.
declaration of performance with respect to its essential
characteristics according to EN 13245-2:2008, Plastics -
The linings are available in all window sizes and generations
Unplasticized poly(vinyl chloride) (PVC-U) profiles for building
sold after 1991.
applications - Part 2: PVC-U profiles and PVC-UE profiles for
internal and external wall and ceiling finishes.
Installation angle: Linings can be installed in roof pitches from
15° to 90°. Base materials/Ancillary materials
Name Value Unit
Plastics 97.7 %
For the placing on the market of the product in the European
Union/European Free Trade Association (EU/EFTA) (with the Steel 2.3 %
exception of Switzerland) Regulation (EU) No. 305/2011 (CPR) REACH
applies. The product needs a declaration of performance taking
into consideration EN 13245-2:2008, Plastics - Unplasticized This product contains substances listed in the candidate list
poly(vinyl chloride) (PVC-U) profiles for building applications - (date: 09.08.2023) exceeding 0.1 percentage by mass: no.
Part 2: PVC-U profiles and PVC-UE profiles for internal and
external wall and ceiling finishes and the CE-marking. Reference service life
A calculation of the reference service life according to ISO
For the application and use the respective national provisions 15686 is not possible.
apply.
The Bundesinstitut für Bau, Stadt und Raumforschung/Federal
Application
office for building and regional planning (BBSR) table declares
Standard linings tobe used in roofs with a roof thickness of min a service life for the complete roof window dependent on the
170 mm to max 530 mm. applied window frame material between 25 and ≥ 50 years.
This includes linings as declared with this EPD.
LCA: Calculation rules
and steel) and their processing (estimated energy data:
Declared Unit electrical energy from the national residual mix and thermal
The declared unit is one m² related to a reference window, that energy from natural gas); transport of major materials to the
the lining is installed in connection with. manufacturing site; assembly of semi-finished products to the
The declared unit is based on the representative product final product; packaging material (including waste paper input
measuring 0.78m x 1.178m. for paper and cardboard).
Declared unit and mass reference
End-of-Life stage C1, C2, C3:
Name Value Unit
C1: a manual demolition is assumed, resulting in indicator value
Declared unit 1 m2 "0".
Grammage 12.56 kg/m2 C2: For the transport to EoL by truck a distance of 50 km is
Layer thickness 0 m assumed.
C3: A scenario for the incineration of plastic in a waste
Weight per area 11.56 kg/representative product
incineration plant (WIP) is assumed; metals are assumed to be
Weight per area 12.56 kg/declared unit
recycled.
The calculation is based mainly on BOM (Bill of Material) data,
with only a few specific The EoL-Scenario does not assume waste to be disposed of on
information on processing. This may lead to a higher a landfill site. Module C4 is declared as"0".
uncertainty for the result values and needs to be kept in mind
for the application of this EPD. Benefits for the next product system D:
Resulting electrical and thermal energy from the WIP, avoiding
System boundary the generation of electricity and heat via fossil fuels, is
Type of EPD: Cradle to gate - with options. The following life considered.
cycle stages were considered: The amount of metals after the reduction due to the net-flow
calculations is sent to a recycling process. The effort for
Production stage A1-A3: recycling, as well as the benefit for the regained metals are
Consideration of the production of raw materials (plastic profile declared in module D.
2 Environmental Product Declaration - VELUX A/S - VELUX lining LSB
Contribution of waste flows is considered in the modules where Comparability
they occur. Basically, a comparison or an evaluation of EPD data is only
possible if all the data sets to be compared were created
Geographic Representativeness according to EN 15804 and the building context, respectively
Land or region, in which the declared product system is the product-specific characteristics of performance, are taken
manufactured, used or handled at the end of the product´s into account. The software LCA FE 10.7 is used accompanied
lifespan: Europe by the MLC database (version 2023.1, 2023).
LCA: Scenarios and additional technical information
Characteristic product properties of biogenic carbon
The following declared values refer to the declared unit of 1 m².
Information on describing the biogenic carbon content at
factory gate
The declared biogenic content comprises the paper manual
and the packaging material consisting of cardboard, paper, PE, Reference service life
EPS and wood. As module A5 is not declared, the information Name Value Unit
on packaging supports further EoL calculations.
Life Span (according to BBSR) 25 - 50 a
Name ValueUnit
kg End of life (C1-C4)
Biogenic carbon content in product -
C Name Value Unit
Biogenic carbon content in accompanying kg Collected separately waste type 12.56 kg
0.8
packaging C Recycling 0.29 kg
The value refers to the following packaging material (per 1m²): Energy recovery 12.27 kg
Paper (manual): 0.08 kg,
Cardboard packaging: 1.429 kg, Reuse, recovery and/or recycling potentials (D), relevant
Paper insert: 0.004 kg, scenario information
PE-LD: 0.057 kg, Name Value Unit
EPS: 0.166 kg, Steel (net-flow-calculation) 0.20 kg/1m² product
wood: 0.217 kg.
Stainless steel (net-flow-calculation) 0.07 kg/1m² product
Note: 1 kg of biogenic carbon is equivalent to 44/12 kg of CO .
2
3 Environmental Product Declaration - VELUX A/S - VELUX lining LSB
LCA: Results
The LCIA assessment is performed applying the characterisation factors "EN 15804+A2, EF 3.0".
DESCRIPTION OF THE SYSTEM BOUNDARY (X = INCLUDED IN LCA; MND = MODULE OR INDICATOR NOT DECLARED; MNR
= MODULE NOT RELEVANT)
Benefits and
Construction loads beyond
Product stage Use stage End of life stage
process stage the system
boundaries
la ire ta m w a Ry lp p u s tro p s n a rT g n iru tc a fu n a M e h t m o rf tro p s n a rTe tis e h t o t e ta g y lb m e s s A e s U e c n a n e tn ia M ria p e R tn e m e c a lp e R tn e m h s ib ru fe R y g re n e la n o ita re p Oe s u re ta w la n o ita re p Oe s u n o itc u rts n o c -e Dn o itilo m e d tro p s n a rT g n is s e c o rp e ts a W la s o p s iD -e s u e R-y re v o c e R-g n ilc y c e Rla itn e to p
A1 A2 A3 A4 A5 B1 B2 B3 B4 B5 B6 B7 C1 C2 C3 C4 D
X X X MND MND MND MND MNR MNR MNR MND MND X X X X X
RESULTS OF THE LCA - ENVIRONMENTAL IMPACT according to EN 15804+A2: 1 m² lining LSB
Parameter Unit A1-A3 C1 C2 C3 C4 D
Global Warming Potential total (GWP-total) kg CO 2 eq 4.24E+01 0 4.84E-02 2.48E+01 0 -8.1E+00
Global Warming Potential fossil fuels (GWP-fossil) kg CO 2 eq 4.23E+01 0 4.6E-02 2.48E+01 0 -8.06E+00
Global Warming Potential biogenic (GWP-biogenic) kg CO 2 eq 8.02E-02 0 2.01E-03 3.91E-03 0 -3.95E-02
Global Warming Potential luluc (GWP-luluc) kg CO 2 eq 3.54E-02 0 4.19E-04 1.71E-03 0 -1.52E-03
Depletion potential of the stratospheric ozone layer (ODP) kg CFC11 eq 2.83E-10 0 5.88E-15 1.61E-11 0 -5.68E-11
Acidification potential of land and water (AP) mol H+ eq 6.77E-02 0 9.08E-05 5.21E-03 0 -1.22E-02
Eutrophication potential aquatic freshwater (EP-freshwater) kg P eq 1.38E-04 0 1.65E-07 4.7E-06 0 -1.24E-05
Eutrophication potential aquatic marine (EP-marine) kg N eq 2.06E-02 0 3.75E-05 1.67E-03 0 -3.12E-03
Eutrophication potential terrestrial (EP-terrestrial) mol N eq 2.23E-01 0 4.27E-04 2.25E-02 0 -3.32E-02
Formation potential of tropospheric ozone photochemical oxidants kg NMVOC
9.71E-02 0 8.12E-05 4.76E-03 0 -8.95E-03
(POCP) eq
Abiotic depletion potential for non fossil resources (ADPE) kg Sb eq 2.38E-05 0 2.98E-09 1.42E-07 0 -1.96E-06
Abiotic depletion potential for fossil resources (ADPF) MJ 9.54E+02 0 6.16E-01 3.59E+01 0 -1.42E+02
m3 world eq
Water use (WDP) 3.46E+00 0 5.46E-04 2.43E+00 0 -9.13E-01
deprived
RESULTS OF THE LCA - INDICATORS TO DESCRIBE RESOURCE USE according to EN 15804+A2: 1 m² lining LSB
Parameter Unit A1-A3 C1 C2 C3 C4 D
Renewable primary energy as energy carrier (PERE) MJ 1.71E+02 0 4.48E-02 8.53E+00 0 -3.95E+01
Renewable primary energy resources as material utilization
MJ 6.57E+00 0 0 -1.25E-01 0 0
(PERM)
Total use of renewable primary energy resources (PERT) MJ 1.78E+02 0 4.48E-02 8.4E+00 0 -3.95E+01
Non renewable primary energy as energy carrier (PENRE) MJ 7E+02 0 6.18E-01 2.81E+02 0 -1.42E+02
Non renewable primary energy as material utilization (PENRM) MJ 2.54E+02 0 0 -2.45E+02 0 0
Total use of non renewable primary energy resources (PENRT) MJ 9.54E+02 0 6.18E-01 3.59E+01 0 -1.42E+02
Use of secondary material (SM) kg 1.47E+00 0 0 0 0 2.71E-01
Use of renewable secondary fuels (RSF) MJ 0 0 0 0 0 0
Use of non renewable secondary fuels (NRSF) MJ 0 0 0 0 0 0
Use of net fresh water (FW) m3 2.15E-01 0 4.91E-05 6.07E-02 0 -3.94E-02
RESULTS OF THE LCA – WASTE CATEGORIES AND OUTPUT FLOWS according to EN 15804+A2:
1 m² lining LSB
Parameter Unit A1-A3 C1 C2 C3 C4 D
Hazardous waste disposed (HWD) kg 1.62E-05 0 1.91E-12 1.29E-10 0 -4.37E-05
Non hazardous waste disposed (NHWD) kg 1.91E+00 0 9.43E-05 9.51E+00 0 -1.3E-02
Radioactive waste disposed (RWD) kg 3.28E-02 0 1.16E-06 1.01E-03 0 -1.03E-02
Components for re-use (CRU) kg 0 0 0 0 0 0
Materials for recycling (MFR) kg 0 0 0 2.9E-01 0 0
Materials for energy recovery (MER) kg 0 0 0 0 0 0
Exported electrical energy (EEE) MJ 4.89E+00 0 0 3.43E+01 0 0
Exported thermal energy (EET) MJ 8.86E+00 0 0 6.2E+01 0 0
RESULTS OF THE LCA – additional impact categories according to EN 15804+A2-optional:
1 m² lining LSB
Parameter Unit A1-A3 C1 C2 C3 C4 D
Disease
Incidence of disease due to PM emissions (PM) 6.9E-07 0 5.87E-10 1.13E-07 0 -1.39E-07
incidence
Human exposure efficiency relative to U235 (IR) kBq U235 eq 4.88E+00 0 1.73E-04 1.23E-01 0 -1.71E+00
Comparative toxic unit for ecosystems (ETP-fw) CTUe 4.63E+02 0 4.37E-01 2.34E+01 0 -3.23E+01
Comparative toxic unit for humans (carcinogenic) (HTP-c) CTUh 2.51E-07 0 8.96E-12 9.92E-10 0 -7.44E-09
4 Environmental Product Declaration - VELUX A/S - VELUX lining LSB
Comparative toxic unit for humans (noncarcinogenic) (HTP-nc) CTUh 4.87E-07 0 5.05E-10 9.44E-08 0 -5.37E-08
Soil quality index (SQP) SQP 2.76E+02 0 2.57E-01 7.7E+00 0 -2.61E+01
Disclaimer 1 – for the indicator 'Potential Human exposure efficiency relative to U235'. This impact category deals mainly with the
eventual impact of low-dose ionizing radiation on human health of the nuclear fuel cycle. It does not consider effects due to possible
nuclear accidents, occupational exposure or radioactive waste disposal in underground facilities. Potential ionizing radiation from the
soil, radon and from some construction materials is also not measured by this indicator.
Disclaimer 2 – for the indicators 'abiotic depletion potential for non-fossil resources', 'abiotic depletion potential for fossil resources',
'water (user) deprivation potential, deprivation-weighted water consumption', 'potential comparative toxic unit for ecosystems', 'potential
comparative toxic unit for humans – cancerogenic', 'Potential comparative toxic unit for humans - not cancerogenic', 'potential soil
quality index'. The results of this environmental impact indicator shall be used with care as the uncertainties on these results are high
as there is limited experience with the indicator.
Disclaimer 3 – for 'potential soil quality index'. Due to a data lack in the foreground data of VELUX, the result has a very high
uncertainty and refers only to the background data, which contain respective information.
References
2.0, Berlin: Institut Bauen und Umwelt e.V., 2021
Standards www.ibu-epd.com
EN 15804
EN 15804:2012+A2:2019+AC:2021, Sustainability of LCA FE 10.7 / MLC DB
construction works — Environmental Product Declarations — Sphera's LCA Software for Experts / Managed LCA Content
Core rules for the product category of construction products. database, Sphera Solutions GmbH, Leinfelden-Echterdingen,
database version 2023.1, 2023
ISO 14025
EN ISO 14025:2011, Environmental labels and declarations —
Type III environmental declarations — Principles and PCR part A
procedures. Calculation Rules for the Life Cycle Assessment and
Requirements on the Project Report according to EN
ISO 15686 15804+A2:2019, version 1.3, IBU, 2022
ISO 15686-1:2011-05: Buildings and constructed assets -
Service life planning
PCR part B
Requirements on the EPD for Windows and doors, version
EN 13245 01.08.2021, IBU
EN 13245-2:2008: Plastics - Unplasticized poly(vinyl chloride)
(PVC-U) profiles for building applications - Part 2: PVC-U REACH/candidate list
profiles and PVC-UE profiles for internal and external wall and Regulation (EC) No 1907/2006: Registration, Evaluation,
ceiling finishes Authorisation and Restriction of Chemicals (REACH)
Regulation (EU) No. 305/2011 (CPR)
Further References Regulation (EU) No 305/2011 of the European Parliament and
of the
BBSR Council of 9 March 2011 laying down harmonised conditions for
BBSR, 24.02.2017, Nutzungsdauer von Bauteilen nach BNB the marketing of construction products and repealing Council
Directive 89/106/EEC Text with EEA relevance
IBU 2021
Institut Bauen und Umwelt e.V.: General Instructions for the
EPD programme of Institut Bauen und Umwelt e.V., Version
5 Environmental Product Declaration - VELUX A/S - VELUX lining LSB
Publisher
Institut Bauen und Umwelt e.V. +49 (0)30 3087748- 0
Hegelplatz 1 info@ibu-epd.com
10117 Berlin www.ibu-epd.com
Germany
Programme holder
Institut Bauen und Umwelt e.V. +49 (0)30 3087748- 0
Hegelplatz 1 info@ibu-epd.com
10117 Berlin www.ibu-epd.com
Germany
Author of the Life Cycle Assessment
Daxner & Merl GmbH +43 676 849477826
Schleifmühlgasse 13/24 office@daxner-merl.com
1040 Wien www.daxner-merl.com
Austria
Angela Schindler Umweltberatung 07553 919 9456
Tüfinger Str. 12 angela@schindler-umwelt.de
88682 Salem www.schindler-umwelt.de
Germany
Owner of the Declaration
VELUX Group +4545164726
Ådalsvej 99 jakob.roerbech@velux.com
2970 Hørsholm www.velux.com
Denmark
6 Environmental Product Declaration - VELUX A/S - VELUX lining LSB
