ENVIRONMENTAL PRODUCT DECLARATION
as per ISO 14025 and EN 15804+A2
Owner of the Declaration VELUX Group
Publisher Institut Bauen und Umwelt e.V. (IBU)
Programme holder Institut Bauen und Umwelt e.V. (IBU)
Declaration number EPD-VEL-20220115-CBB3-EN
Issue date 24.05.2022
Valid to 23.05.2027
Collar BBX
Velux
www.ibu-epd.com | https://epd-online.com
General Information
Velux Collar BBX
Programme holder Owner of the declaration
IBU – Institut Bauen und Umwelt e.V. VELUX Group
Hegelplatz 1 Ådalsvej 99
10117 Berlin 2970 Hørsholm
Germany Denmark
Declaration number Declared product / declared unit
EPD-VEL-20220115-CBB3-EN 1m² water vapour barrier BBX
The declared unit is based on the configuration of a standard size window
measuring 0.78m x 1.178m.
This declaration is based on the product category rules: Scope:
Windows and doors , 01.08.2021 Productline BBX - Collar/installation product; manufactured by VELUX in
(PCR checked and approved by the SVR) China for sale in Europe.
Declaration according to ISO 14025 and EN 15804 describing specific
Issue date environmental performances of the construction product.
The owner of the declaration shall be liable for the underlying information
24.05.2022
and evidence; the IBU shall not be liable with respect to manufacturer
information, life cycle assessment data and evidences.
Valid to
The EPD was created according to the specifications of EN 15804+A2. In
23.05.2027 the following, the standard will be simplified as EN 15804.
Verification
The standard EN 15804 serves as the core PCR
Independent verification of the declaration and data according to ISO
14025:2011
internally X externally
Dipl.-Ing. Hans Peters
(Chairman of Institut Bauen und Umwelt e.V.)
Florian Pronold Prof. Dr. Birgit Grahl,
(Managing Director Institut Bauen und Umwelt e.V.) (Independent verifier)
1 Environmental Product Declaration - Velux - Collar BBX
Product
Performance data of the product in accordance with the
Product description/Product definition declaration of performance with respect to its essential
The VELUX BBX water vapour barrier is a product for sale in characteristics according to DIN EN 13984:2013, Flexible
the European market. sheets for waterproofing – Plastic and rubber vapour control
layers – Definitions and characteristics - Part 1: Windows and
All the vapour barriers consist of mainly plastics. external pedestrian doorsets.
The calculations are based on the BBX water vapour barrier. Base materials/Ancillary materials
For the placing on the market of the product in the European Name Value Unit
Union/European Free Trade Association (EU/EFTA) (with the
Galvanized steel 1 %
exception of Switzerland) Regulation (EU) No. 305/2011 (CPR)
Polyethylene LD 99 %
applies. The product needs a declaration of performance taking
into consideration DIN EN 13984:2013, Flexible sheets for
waterproofing – Plastic and rubber vapour control layers – REACH
Definitions and characteristics. For the application and use, the
respective national provisions apply.. This product/article/at least one partial article contains
substances listed in the candidate list (date: 17.01.2022)
Application exceeding 0.1 percentage by mass: no.
VELUX BBX water vapour barriers used in renovation and new
build. Recycled content
Technical Data
The Declaration of Performance including relevant technical
specifications and test methods/test standards can be
downloaded from the website www.velux.com/ce-marking.
The values stated in the table relate to the recycled material
The performance values are specific for the BBX water vapour streams in VELUX production.
barrier.
Reference service life
The declared values in the table relate to the reference product. A calculation of the reference service life according to ISO
For other covered product variants, specific values can be 15686 is not possible.
selected at the bottom of the above-mentioned download page.
The Bundesinstitut für Bau, Stadt und Raumforschung/Federal
office for building and regional planning (BBSR)
Constructional data
table declares for the complete roof window a service life
Name Value Unit
dependent on the applied window frame material between 25
Fire resistance class DIN EN 1634-1 E class and ≥ 50 years. This includes collars and flashings as declared
Water tightness test is passed with this EPD.
Water vapour resistance, Sd = 80 m
LCA: Calculation rules
cardboard).
Declared Unit
The declared unit is one m² related to a reference window, that End-of-Life stage C1, C2, C3:
the collar is installed in connection with.
C1: a manual demolition is assumed, resulting in indicator value
The declared unit is based on the representative product "0".
measuring 0.78m x 1.178m. C2: For the transport to EoL by truck a distance of 50 km is
Declared unit assumed.
C3: A scenario for the incineration of plastics in a waste
Name Value Unit
incineration plant (WIP) is assumed.
Declared unit 1 m2
Weight per area 0.82 kg/representative product The EoL-Scenario does not assume waste to be disposed of on
Weight per area 0.89 kg/declared unit a landfill site. Module C4 is declared as "0".
Benefits for the next product system D:
Resulting electrical and thermal energy from the WIP, avoiding
System boundary
the generation of electricity and heat via fossil fuels, is
Type of EPD: Cradle to gate - with options. The following life
considered.
cycle stages were considered:
The amount of metals after the reduction due to the net-flow
calculations is sent to a recycling process. The effort for
Production stage A1-A3:
recycling, as well as the benefit for the regained metals are
Consideration of the production of raw materials and their
declared in module D.
processing; transport of major material to the manufacturing
site; assembly of semi-finished products to the final product;
Contribution of waste flows is considered in the modules where
packaging material (including waste paper input for paper and
they occur.
2 Environmental Product Declaration - Velux - Collar BBX
Basically, a comparison or an evaluation of EPD data is only
Geographic Representativeness possible if all the data sets to be compared were created
Land or region, in which the declared product system is according to EN 15804 and the building context, respectively
manufactured, used or handled at the end of the product´s the product-specific characteristics of performance, are taken
lifespan: Europe into account. The software GaBi is used accompanied by the
GaBi background data base (version 2021.2, 2021).
Comparability
LCA: Scenarios and additional technical information
Characteristic product properties of biogenic carbon
The following declared values refer to the declared unit of 1m².
Information on describing the biogenic Carbon Content at
factory gate Reference service life
The declared biogenic content comprises the paper manual Name Value Unit
and the packaging material consisting of cardboard, paper and
Life Span (according to BBSR) depending on 25 -
wood. As module A5 is not declared, the information on a
window frame material 50
packaging supports further EoL calculations.
Name ValueUnit End of life (C1-C4)
kg Name Value Unit
Biogenic carbon content in product -
C Collected separately waste type waste type 0.89 kg
Biogenic carbon content in accompanying 0.116 kg Recycling 0.005 kg
packaging C
Energy recovery 0.88 kg
The value refers to the following packaging material (per 1m²):
Paper (manual): 0.005kg, Cardboard packaging: 0.248kg, Reuse, recovery and/or recycling potentials (D), relevant
Paper insert: 0.003kg, PE-LD: 0.034kg, Wood: 0,011kg scenario information
Name Value Unit
Note: 1 kg of biogenic carbon is equivalent to 44/12 kg of CO .
2 Steel (net-flow calculation) 7.21E-03 kg/1m² product
3 Environmental Product Declaration - Velux - Collar BBX
LCA: Results
DESCRIPTION OF THE SYSTEM BOUNDARY (X = INCLUDED IN LCA; MND = MODULE OR INDICATOR NOT DECLARED; MNR
= MODULE NOT RELEVANT)
Benefits and
Construction loads beyond
Product stage Use stage End of life stage
process stage the system
boundaries
la ire ta m w a Ry lp p u s tro p s n a rT g n iru tc a fu n a M e h t m o rf tro p s n a rTe tis e h t o t e ta g y lb m e s s A e s U e c n a n e tn ia M ria p e R tn e m e c a lp e R tn e m h s ib ru fe R y g re n e la n o ita re p Oe s u re ta w la n o ita re p Oe s u n o itc u rts n o c -e Dn o itilo m e d tro p s n a rT g n is s e c o rp e ts a W la s o p s iD -e s u e R-y re v o c e R-g n ilc y c e Rla itn e to p
A1 A2 A3 A4 A5 B1 B2 B3 B4 B5 B6 B7 C1 C2 C3 C4 D
X X X MND MND MND MND MNR MNR MNR MND MND X X X X X
RESULTS OF THE LCA - ENVIRONMENTAL IMPACT according to EN 15804+A2: 1 m² BBX
Parameter Unit A1-A3 C1 C2 C3 C4 D
Global Warming Potential total (GWP-total) kg CO 2 eq 4.39E+00 0 2.7E-03 2.21E+00 0 -1.15E+00
Global Warming Potential fossil fuels (GWP-fossil) kg CO 2 eq 4.8E+00 0 2.68E-03 2.21E+00 0 -1.14E+00
Global Warming Potential biogenic (GWP-biogenic) kg CO 2 eq -4.06E-01 0 -3.19E-06 1.4E-04 0 -5.68E-03
Global Warming Potential luluc (GWP-luluc) kg CO 2 eq 2.74E-03 0 2.19E-05 8.42E-05 0 -7.85E-04
Depletion potential of the stratospheric ozone layer (ODP) kg CFC11 eq 3.67E-12 0 5.29E-19 6.79E-16 0 -1.3E-14
Acidification potential of land and water (AP) mol H+ eq 1.22E-02 0 5.29E-06 2.83E-04 0 -1.5E-03
Eutrophication potential aquatic freshwater (EP-freshwater) kg P eq 1.43E-05 0 7.96E-09 1.05E-07 0 -1.49E-06
Eutrophication potential aquatic marine (EP-marine) kg N eq 3.19E-03 0 2.19E-06 7.7E-05 0 -4.25E-04
Eutrophication potential terrestrial (EP-terrestrial) mol N eq 3.4E-02 0 2.49E-05 1.29E-03 0 -4.55E-03
Formation potential of tropospheric ozone photochemical oxidants kg NMVOC
1.1E-02 0 4.72E-06 2.22E-04 0 -1.2E-03
(POCP) eq
Abiotic depletion potential for non fossil resources (ADPE) kg Sb eq 5.91E-07 0 2.38E-10 9.83E-09 0 -2.16E-07
Abiotic depletion potential for fossil resources (ADPF) MJ 1.03E+02 0 3.57E-02 8.62E-01 0 -1.98E+01
m3 world eq
Water use (WDP) 1.63E+00 0 2.49E-05 2.3E-01 0 -1.17E-01
deprived
RESULTS OF THE LCA - INDICATORS TO DESCRIBE RESOURCE USE according to EN 15804+A2: 1 m² BBX
Parameter Unit A1-A3 C1 C2 C3 C4 D
Renewable primary energy as energy carrier (PERE) MJ 4.37E+00 0 2.05E-03 1.87E-01 0 -4.45E+00
Renewable primary energy resources as material utilization
MJ 4.27E+00 0 0 0 0 0
(PERM)
Total use of renewable primary energy resources (PERT) MJ 8.64E+00 0 2.05E-03 1.87E-01 0 -4.45E+00
Non renewable primary energy as energy carrier (PENRE) MJ 6.33E+01 0 3.58E-02 4.12E+01 0 -1.98E+01
Non renewable primary energy as material utilization (PENRM) MJ 4.03E+01 0 0 -4.03E+01 0 0
Total use of non renewable primary energy resources (PENRT) MJ 1.04E+02 0 3.58E-02 8.63E-01 0 -1.98E+01
Use of secondary material (SM) kg 2.28E-01 0 0 0 0 6.5E-03
Use of renewable secondary fuels (RSF) MJ 0 0 0 0 0 0
Use of non renewable secondary fuels (NRSF) MJ 0 0 0 0 0 0
Use of net fresh water (FW) m3 4.17E-02 0 2.35E-06 5.45E-03 0 -5.06E-03
RESULTS OF THE LCA – WASTE CATEGORIES AND OUTPUT FLOWS according to EN 15804+A2:
1 m² BBX
Parameter Unit A1-A3 C1 C2 C3 C4 D
Hazardous waste disposed (HWD) kg 8.72E-08 0 1.89E-12 1.54E-10 0 -4.4E-09
Non hazardous waste disposed (NHWD) kg 6.57E-02 0 5.62E-06 2.13E-01 0 -7.87E-03
Radioactive waste disposed (RWD) kg 9.78E-04 0 6.5E-08 3.36E-05 0 -1.43E-03
Components for re-use (CRU) kg 0 0 0 0 0 0
Materials for recycling (MFR) kg 0 0 0 4.9E-03 0 0
Materials for energy recovery (MER) kg 0 0 0 0 0 0
Exported electrical energy (EEE) MJ 0 0 0 4.89E+00 0 0
Exported thermal energy (EET) MJ 0 0 0 8.82E+00 0 0
RESULTS OF THE LCA – additional impact categories according to EN 15804+A2-optional:
1 m² BBX
Parameter Unit A1-A3 C1 C2 C3 C4 D
Disease
Incidence of disease due to PM emissions (PM) 1.45E-07 0 3.21E-11 4E-09 0 -1.31E-08
incidence
Human exposure efficiency relative to U235 (IR) kBq U235 eq 1.17E-01 0 9.5E-06 4.4E-03 0 -2.35E-01
Comparative toxic unit for ecosystems (ETP-fw) CTUe 4.53E+01 0 2.65E-02 6.16E-01 0 -4.14E+00
Comparative toxic unit for humans (carcinogenic) (HTP-c) CTUh 1.39E-09 0 5.36E-13 3.35E-11 0 -1.94E-10
4 Environmental Product Declaration - Velux - Collar BBX
Comparative toxic unit for humans (noncarcinogenic) (HTP-nc) CTUh 5.08E-08 0 2.91E-11 3.61E-09 0 -7.54E-09
Soil quality index (SQP) SQP 2.09E+01 0 1.23E-02 2.1E-01 0 -3.05E+00
Disclaimer 1 – for the indicator 'Potential Human exposure efficiency relative to U235'.
This impact category deals mainly with the eventual impact of low dose ionizing radiation on human health of the nuclear fuel cycle. It
does not consider effects due to possible nuclear accidents, occupational exposure or radioactive waste disposal in underground
facilities. Potential ionizing radiation from the soil, radon and from some construction materials is also not measured by this indicator.
Disclaimer 2 – for the indicators 'abiotic depletion potential for non-fossil resources', 'abiotic depletion potential for fossil resources',
'water (user) deprivation potential, deprivation-weighted water consumption', 'potential comparative toxic unit for ecosystems', 'potential
comparative toxic unit for humans – cancerogenic', 'Potential comparative toxic unit for humans - not cancerogenic', 'potential soil
quality index'. The results of this environmental impact indicator shall be used with care as the uncertainties on these results are high
or as there is limited experience with the indicator.
Disclaimer 3 – for 'potential soil quality index'. Due to a data lack in the foreground data of VELUX, the result has a very high
uncertainty and refers only to the background data, which contain respective information.
References
BBSR ISO 14025
BBSR, 24.02.2017, Nutzungsdauer von Bauteilen nach BNB EN ISO 14025:2011, Environmental labels and declarations —
Type III environmental declarations — Principles and
DIN EN 1634-1 procedures.
DIN EN 1634-1:2018-04: Fire resistance and smoke control
tests for door and shutter assemblies, openable windows and ISO 15686
elements of building hardware - Part 1: Fire resistance test for ISO 15686:2011-05: Buildings and constructed assets - Service
door and shutter assemblies and openable windows life planning - Part 1: General principles and framework
DIN EN 13984 PCR part A
DIN EN 13984:2013-05: Flexible sheets for waterproofing - Calculation Rules for the Life Cycle Assessment and
Plastic and rubber vapour control layers - Definitions and Requirements on the Project Report according to EN
characteristics 15804+A2:2019, version 1.2, Berlin: Institut Bauen und Umwelt
e.V., 2021
EN 15804
EN 15804:2012+A2:2019, Sustainability of construction works PCR part B
— Environmental Product Declarations — Core rules for the Requirements on the EPDS for Windows and doors, version
product category of construction products. 01-2021, Berlin: Institut Bauen und Umwelt e.V.
GaBi REACH
GaBi Software and GaBi Database by Sphera Solution GmbH, Regulation (EC) No 1907/2006 of the European Parliament and
version: 2021.2, 2021 of the Council on the Registration, Evaluation, Authorisation
and Restriction of Chemicals (REACH)
IBU 2021
Institut Bauen und Umwelt e.V.: General Instructions for the Regulation (EU) No. 305/2011 (CPR)
EPD programme of Institut Bauen und Umwelt e.V., Version Regulation (EU) No 305/2011 of the European Parliament and
2.0, Berlin: Institut Bauen und Umwelt e.V., 2021, www.ibu- of the Council of 9 March 2011 laying down harmonized
epd.com conditions for the marketing of construction products and
repealingCounsicl Directive 89/106/EEC
5 Environmental Product Declaration - Velux - Collar BBX
Publisher
Institut Bauen und Umwelt e.V. +49 (0)30 3087748- 0
Hegelplatz 1 info@ibu-epd.com
10117 Berlin www.ibu-epd.com
Germany
Programme holder
Institut Bauen und Umwelt e.V. +49 (0)30 3087748- 0
Hegelplatz 1 info@ibu-epd.com
10117 Berlin www.ibu-epd.com
Germany
Author of the Life Cycle Assessment
Daxner & Merl GmbH +43 676 849477826
Lindengasse 39/8 office@daxner-merl.com
1070 Wien www.daxner-merl.com
Austria
Angela Schindler Umweltberatung 07553 919 9456
Tüfinger Str. 12 angela@schindler-umwelt.de
88682 Salem www.schindler-umwelt.de
Germany
Owner of the Declaration
VELUX Group +4545164726
Ådalsvej 99 jakob.roerbech@velux.com
2970 Hørsholm www.velux.com
Denmark
6 Environmental Product Declaration - Velux - Collar BBX
