1114
NEPD
Ver. 2 2015(17)
ENVIRONMENTAL PRODUCT DECLARATION
in accordance with ISO 14025, ISO 21930 and EN 15804
Owner of the declaration: Fibo AS
Program operator: The Norwegian EPD Foundation
Publisher: The Norwegian EPD Foundation
Declaration number: NEPD-2105-950-EN
Registration number: NEPD-2105-950-EN
ECO Platform reference number: -
Issue date: 17.03.2020
Valid to: 17.03.2025 (validity extended to 31.03.2025)
Fibo wall panels
Fibo AS
www.epd-norge.no
NEPD-2105-950-EN Fibo wall panels
General information
Product: Owner of the declaration:
Fibo wall panels Fibo AS
Contact person: Elise Almås
Phone: +47 38 34 33 00
e-mail: eal@fibosystem.com
Program operator: Manufacturer:
Norwegian EPD Foundation Fibo AS
P.O. Box 5250 Majorstuen, 0303 Oslo Industriveien 2, NO-4580 Lyngdal
Phone: +47 97722020 Norway
e-mail: post@epd-norge.no
Declaration number: Place of production:
NEPD-2105-950-EN Lyngdal, Norway
ECO Platform reference number: Management system:
NS-EN ISO 9001:2015, PEFC ST 2002:2013
This declaration is based on Product Category Rules: Organisation no:
CEN Standard EN 15804 serves as core PCR NO 964 193 991 MVA
NPCR 010:2019 Part B for Building boards version 3
Statement of liability: Issue date:
The owner of the declaration shall be liable for the 17.03.2020
underlying information and evidence. EPD Norway shall
not be liable with respect to manufacturer information, life
cycle assessment data and evidences.
Valid to:
17.03.2025 (validity extended to 31.03.2025)
Declared unit: Year of study:
2019
Declared unit with option: Comparability:
1 m2 covering surface of installed wall panel with an EPD of construction products may not be comparable if they
thickness of 10.2 mm and an expected lifetime of 20 years, do not comply with EN 15804 and are seen in a building
including installation, maintenance and waste treatment at context.
end-of-life.
Functional unit: The EPD has been worked out by:
Vegard Ruttenborg
Norwegian Institute of Wood Technology
Verification:
The CEN Norm EN 15804 serves as the core PCR.
Independent verification of the declaration and data,
according to ISO14025:2010
internal external
Approved
Third party verifier:
Fredrik Moltu Johnsen, PhD, Østfoldforskning AS
(Independent verifier approved by EPD Norway)
NEPD-2105-950-EN Fibo wall panels
2/9
Product
Product description: Technical data:
Fibo wall panels are a waterproof panel system based on Plywood has 7 layers of veener in accordance to NS-EN
plywood covered with high-pressure laminate (HPL) on 13986 with water resistant glue, a thickness of 9 mm and a
the front and a thinner balancing layer on the back. density of 680 kg/m3. HPL in accordance to EN 438-3 with a
thickness of 0.6-0.8 mm on the frontside and a balancing
Fibo wall panels can be used as water proof layer on walls layer of 0.2-0.3 mm on the backside. The density of the HPL
in bathrooms. The panels are also suitable for wardrobes, is 1350 kg/m3.
washing rooms, cleaning rooms, laboratories, commercial
kitchens, sport facilities, camping sites, hotels, schools,
Market:
etc.
Norway, Northern Europe and North America. The
scenarios are based on the Norwegian market.
Product specification: Reference service life, product:
Wall panels are made both as bathroom panels in a size of 60 As a conservative scenario, the service life of the wall panel
cm x 240 cm and as kitchen board in a size of 60 cm x 58 cm. is set to 20 years. The estimated service lifetime is provided
by the manufacturer. There is no available documentation
for this estimation. With good maintenance of sealant in
Materials kg % profiles, the service life of the panels can be extended,
Birch plywood 6,12 80,74 which means there will be no need for replacement of the
High-pressure laminates 1,08 14,25 panels after 20 years.
Glue and hardener 0,14 1,85
Balancing laminates 0,24 3,17
Total product 7,58 100,00
Wood packaging 0,20
Plastic packaging 0,03
Cardboard packaging 0,03
Total with packaging 7,83
LCA: Calculation rules
Declared unit with options: System boundary:
1 m2 covering surface of installed wall panel with an A flow chart with the system bounadries are shown below in
thickness of 10.2 mm and an expected lifetime of 20 years, figure 1.
including installation, maintenance and waste treatment at
end-of-life. Module D i calculated based on exported energy from waste
processing substituting average electricity and district
heating production.
Figure 1: Flow diagram according to the modular approach.
NEPD-2105-950-EN Fibo wall panels
3/9
Data quality: Cut-off criteria:
Manufacturing data is collected in 2019 and is based on average All major raw materials and all the essential energy is
data for 2018. Data for exported energy from waste processing included. The production process for raw materials and
are based on Statistics Norway and are representative for 2017 energy flows that are included with very small amounts
(2018a, b, c). Data for manufacturing of HPL is collected from an (<1%) are not included. This cut-off rule does not apply for
EPD (IBU, 2017). The remaining data are from Ecoinvent v3.5 hazardous materials and substances.
"Allocation cut-off by classification" (2018), but adjusted to
improve representativeness.
Modelling and LCA calculations is performed with SimaPro
version 9.0.0.48.
Calculation of biogenic carbon content:
Sequestration and emissions of biogenic carbon is
Allocation: calculated according to EN16485:2014. This approach is
The allocation is made ​​in accordance with the provisions of EN based on the modularity principle in EN15804:2012 that
15804. No allocation has been utilized in the production at Fibo states that all environmental aspects and impacts are
AS. All incoming and outgoing materials and energy are declared in the life cycle where they appear. The
allocated to the main product. Allocation in upstream processes calculation of biogenic carbon content and conversion to
is used by default in Ecoinvent v3.5. carbon dioxide is done according to NS-EN 16449:2014. Net
contribution to GWP from biogenic carbon by each module
is shown on page 8. Wood raw materials origins from
sustainable forestry and is PEFC certified (DNV GL, 2019).
LCA: Scenarios and additional technical information
The following information describe the scenarios in the different modules of the EPD:
Transport to building site is based on a scenario with transport from the factory to a builders' merchant in Oslo and then an
additional 30 km to a building site.
Transport from production place to user (A4)
Type Type of vehicle Distance Fuel/Energy Fuel/Energy
Capacity utilisation (incl. return) %
km consumption consumption
Lorry 53 EURO 5, >32 tonnes 400 0.023 l/tkm 0.31 l/km
Lorry 37 EURO 5, 16-32 tonnes 30 0.045 l/tkm 0.25 l/km
Assembly (A5)
Unit Value The assembly at building site includes 10 % product wastage and 1
Sealant kg 0.027 MJ energy per kubic meter for lifting. Waste management of
Aluminium profile kg 0.018 packaging and product wastage is included. In addition, the
Water consumption m3 installation requires sealant and an aluminium profile.
Electricity consumption MJ 0.0102
Other energy carriers MJ
Material loss kg 0.758
Output materials from waste treatment kg 0.25
Dust in the air kg
Maintenance (B2)
Unit Value Visible sealant is expected to be checked for damage annually. These
Maintenance cycle, sealant* yr 3 areas is assumed to require repair during the service life. Examples of
Sealant, total for 3 years mL 50 such areas are shower wardrobes in indoor swimming pools, hotels
Detergent, per year mL 5 etc. If the sealant is required to be removed and replaced by new
Water consumption, per year liter 0.245 sealant it is assumed a consumption of 50 mL per square meter of
Electricity consumption kWh wall panel. In the EPD calculations it is assumed a scenario where the
Other energy carriers MJ sealant is replaced every 3rd year (extreme use). In addition, it is
Material loss kg assumed that visible sealant in wet areas is cleaned with chlorine
water every other month to remove skin and soap residue and to
prevent fungal growth on the sealant. These requirments applies to
both private and public buildings.
Replacement (B4)
Unit Verdi It is used a conservative scenario where the service life of the wall
Replacement cycle* År 20 panels is set to 20 years. During the service life of the building it is
Electricity consumption kWh required to replace the wall panels twice. With good maintenance of
Replacement of worn parts 0 sealant in profiles, the service life of the panels can be longer, which
means there will be no need for replacement of the panels after 20
years.
*Number or RSL (Reference Service Life)
NEPD-2105-950-EN Fibo wall panels
4/9
End of Life (C1, C3, C4)
Unit Value Wall panels are collected as mixed construction waste at
Hazardous waste disposed kg building site and treated with incineration with energy
Collected as mixed construction waste kg 7.58 recovery. Ash from incineraiton is disposed in landfill.
Reuse kg
Recycling kg
Energy recovery kg 7.58
To landfill kg
The transport of wood waste is based on average distance for Norway in 2007 and was 85 km (Raadal et al., 2009).
Transport to waste processing (C2)
Type Type of vehicle Distance Fuel/Energy Fuel/Energy
Capacity utilisation (incl. return) %
km consumption consumption
Lorry 43 Unspecified 85 0.03 l/tkm 0.28 l/km
Benefits and loads beyond the system boundaries (D)
Unit Value The benefits of exported energy from energy recovery is
Substitution of electricity MJ 39,7 calculated with substiution of Norwegian electricity market mix
Substitution of district heating MJ 272,9 on medium voltage and Norwegian district heating mix. The
Substitution of raw materials kg 0,00 energy exported and the district heating mix is representative
for the year 2017.
NEPD-2105-950-EN Fibo wall panels
5/9
LCA: Results
System boundaries (X = included, MND = module not declared, MNR = module not relevant)
MND
Environmental impact
Parameter
POCP
AP
EP
ADPM
ADPE
Environmental impact
tropsnarT
ecnanetniaM
MND
A5
9,17E-08 4,59E-08
7,56E-04 2,43E-03
6,25E-03 1,05E-01
1,18E-03 1,88E-03 2,30E-02
6,45E-07 4,00E-06 5,14E-05
1,51E+02 5,14E+00 2,30E+01 1,49E+02
Parameter Unit B6 B7
POCP
GWP Global warming potential; ODP Depletion potential of the stratospheric ozone layer; POCP Formation potential of tropospheric
photochemical oxidants; AP Acidification potential of land and water; EP Eutrophication potential; ADPM Abiotic depletion potential for non
fossil resources; ADPE Abiotic depletion potential for fossil resources
ylbmessA
End of life stage
A1 A2 A5 B2 B4 B5 C1 C3
X X X X X MND
B1 B2
GWP 2,08E+00 1,10E+01
ODP
6,06E-03 4,95E-05
kg SO 2 -ekv 4,20E-02 9,99E-04 1,95E-02
kg PO 43--ekv 9,10E-03 1,68E-04
2,59E-05
gnirutcafunaM
noitilomed
noitcurtsnoc-eD
Product stage
D
6,05E-08
kg C H -ekv 2 4
kg Sb-ekv 2,06E-05
lasopsiD
-gnilcyceR-yrevoceR-esueR
laitnetop
C4
X
B4
3,24E+01
1,75E-06
1,39E-02
gnissecorp
etsaW
C2
X
B3 B5
tropsnarT
MNR
kg CFC11-ekv 6,96E-07
esU
The results for Global Warming Potential has a large contribution from sequestration of carbon dioxide during wood growth in the
various modules. The uptake of biogenic carbon dioxide in the product in module A1-A3 is 9.8 kg CO per declared unit. The
2
same amount is released back to air in module C3 during incineration. Biogenic carbon stored in packaging is released to air
when the waste packaging is incinerated in A5. The amount of net contribution of biogenic carbon to each module is shown on
page 8.
Beyond the
system
boundaries
A3 A4 B3 B7
X
Unit A1-A3 A4
kg CO -ekv 3,98E-01 3,09E-01
2
riapeR
tnemhsibrufeR
Use stage
MNR
esu
ygrene
lanoitarepO
B1
slairetam
waR
tropsnarT
tnemecalpeR
B6
X X X
esu
retaw
lanoitarepO
Assemby stage
X
MJ 4,17E+02
C1 C2 C3 C4 D
GWP kg CO -ekv 8,99E-05 8,24E-02 1,33E+01 1,12E-03 -3,78E+00
2
ODP kg CFC11-ekv 8,41E-12 1,53E-08 1,29E-08 3,87E-10 -2,30E-07
kg C 2H 4 -ekv 1,86E-08 1,38E-05 8,11E-05 3,03E-07 -1,31E-03
AP kg SO 2 -ekv 4,05E-07 3,23E-04 2,69E-03 7,06E-06 -1,36E-02
EP kg PO 43--ekv 1,01E-07 5,67E-05 9,98E-04 1,29E-06 -3,11E-03
ADPM kg Sb-ekv 1,41E-09 2,32E-07 2,25E-07 1,88E-09 -7,10E-06
ADPE MJ 9,52E-04 1,34E+00 2,83E+01 3,67E-02 -5,16E+01
NEPD-2105-950-EN Fibo wall panels
6/9
Resource use
Parameter Unit A1-A3 A4 A5 B1 B2 B3 B4 B5
RPEE MJ 1,30E+02 8,17E-02 2,53E+01 6,40E+00 5,40E+02
RPEM MJ 1,18E+02 0,00E+00 4,28E-01 0,00E+00 9,42E+00
TPE MJ 2,48E+02 8,17E-02 2,57E+01 6,40E+00 5,50E+02
NRPE MJ 1,65E+02 5,29E+00 2,53E+01 1,27E+02 4,69E+02
NRPM MJ 3,77E+01 0,00E+00 7,47E-01 1,78E-15 5,74E+00
TRPE MJ 2,03E+02 5,29E+00 2,61E+01 1,27E+02 4,75E+02
SM kg 4,41E-03 0,00E+00 4,94E-03 0,00E+00 1,87E-02
RSF MJ 2,38E-01 0,00E+00 8,97E-02 1,26E-01 1,97E+00
NRSF MJ 3,20E-02 0,00E+00 3,60E-02 8,39E-02 7,92E-01
W
m3
2,23E-01 1,03E-03 2,97E-02 6,51E-02 5,29E-01
Resource use
Parameter Unit B6 B7 C1 C2 C3 C4 D
RPEE MJ 1,15E-02 1,72E-02 1,14E+02 5,69E-04 -1,71E+02
RPEM MJ 0,00E+00 0,00E+00 -1,14E+02 0,00E+00 0,00E+00
TPE MJ 1,15E-02 1,72E-02 6,10E-01 5,69E-04 -1,71E+02
NRPE MJ 1,62E-03 1,36E+00 3,75E+01 3,78E-02 -6,30E+01
NRPM MJ 0,00E+00 0,00E+00 -3,56E+01 0,00E+00 0,00E+00
TRPE MJ 1,62E-03 1,36E+00 1,86E+00 3,78E-02 -6,30E+01
SM kg 0,00E+00 0,00E+00 0,00E+00 0,00E+00 0,00E+00
RSF MJ 0,00E+00 0,00E+00 6,59E-01 0,00E+00 -1,06E+02
NRSF MJ 0,00E+00 0,00E+00 3,28E-01 0,00E+00 -7,10E+01
W m3 8,58E-05 2,44E-04 1,04E-02 4,02E-05 -6,83E-01
RPEE Renewable primary energy resources used as energy carrier; RPEM Renewable primary energy resources used as raw materials;
TPE Total use of renewable primary energy resources; NRPE Non renewable primary energy resources used as energy carrier; NRPM Non
renewable primary energy resources used as materials; TRPE Total use of non renewable primary energy resources; SM Use of secondary
materials; RSF Use of renewable secondary fuels; NRSF Use of non renewable secondary fuels; W Use of net fresh water
End of life - Waste
Parameter Unit A1-A3 A4 A5 B1 B2 B3 B4 B5
HW kg 4,89E-02 3,17E-04 1,80E-02 5,40E-02 3,55E-01
NHW kg 1,28E+00 4,09E-01 2,26E-01 8,81E-02 4,10E+00
RW kg 4,77E-04 3,49E-05 6,11E-05 5,16E-06 1,17E-03
End of life - Waste
Parameter Unit B6 B7 C1 C2 C3 C4 D
HW kg 5,73E-07 3,97E-05 7,55E-04 1,09E-01 -1,54E-02
NHW kg 6,87E-05 8,00E-02 2,19E-02 3,49E-02 -6,50E-01
RW kg 1,13E-08 8,63E-06 3,99E-06 2,23E-07 -1,46E-04
HW Hazardous waste disposed; NHW Non hazardous waste disposed; RW Radioactive waste disposed
End of life - Output flow
Parameter Unit A1-A3 A4 A5 B1 B2 B3 B4 B5
CR kg 0,00E+00 0,00E+00 0,00E+00 0,00E+00 0,00E+00
MR kg 2,32E-02 0,00E+00 5,69E-02 0,00E+00 1,71E-01
MER kg 8,00E-03 0,00E+00 2,01E-01 0,00E+00 4,18E-01
EEE MJ 7,11E-01 0,00E+00 1,33E+00 2,80E+00 2,92E+01
ETE MJ 6,64E+00 0,00E+00 8,47E+00 3,15E+01 1,86E+02
End of life - Output flow
Parameter Unit B6 B7 C1 C2 C3 C4 D
CR kg 0,00E+00 0,00E+00 0,00E+00 0,00E+00 0,00E+00
MR kg 0,00E+00 0,00E+00 5,55E-03 0,00E+00 0,00E+00
MER kg 0,00E+00 0,00E+00 0,00E+00 0,00E+00 0,00E+00
EEE MJ 0,00E+00 0,00E+00 1,26E+01 0,00E+00 -3,97E+01
ETE MJ 0,00E+00 0,00E+00 7,80E+01 0,00E+00 -2,73E+02
CR Components for reuse; MR Materials for recycling; MER Materials for energy recovery; EEE Exported electric energy; ETE Exported
thermal energy
Reading example: 9,0 E-03 = 9,0*10-3 = 0,009
NEPD-2105-950-EN Fibo wall panels
7/9
Additional Norwegian requirements
Greenhouse gas emission from the use of electricity in the manufacturing phase
National production mix with import, on low voltage (production of transmission lines, in addition to direct emissions and losses in
grid) is applied for electricity in the manufacturing prosess (A3).
Data source Amount Unit
Ecoinvent v3.5 (August 2018) 31.7 gram CO -eq/kWh
2
Dangerous substances
The product contains no substances given by the REACH Candidate list or the Norwegian priority list
The product contains substances given by the REACH Candidate list or the Norwegian priority list that are less than 0,1 %
by weight.
The product contain dangerous substances, more then 0,1% by weight, given by the REACH Candidate List or the
Norwegian Priority list, see table.
The product contains no substances given by the REACH Candidate list or the Norwegian priority list. The product is
classified as hazardous waste (Avfallsforskiften, Annex III), see table.
Transport
Transport from production site to construction site in Norway according to scenario in module A4: 430 km
Indoor environment
The product meets the requirements for low emissions, M1 (Rise, 2019). See table below for test results.
Sealant FIBOSEAL meets the requirements according to EC 1 Plus (GEV, 2017).
Compounds Requirement M1 Test results Pass / Fail
(mg/m2h)
TVOC < 0,2 0,013 PASS
Formaldehyde < 0,05 0,028 PASS
CMR 1A+1B < 0,005 < 0,001 PASS
Ammonia < 0,03 not measured --
Odour ≥ 0,0 not measured --
Carbon footprint
To increase the transparency of the climate impacts, the GWP indicator has been divided into sub-indicators:
GWP-IOBC Climate impacts calculated according to instant oxidation principle
GWP-BCIP Climate impacts calculated from the net impacts of sequestration and emission of biogenic carbon
Climate impact
Parameter Unit A1-A3 A4 A5 B1 B2 B3 B4 B5
GWP-IOBC kg CO 2 -ekv 1,05E+01 3,09E-01 1,77E+00 1,10E+01 3,25E+01
GWP-BCIP kg CO 2 -ekv -1,01E+01 0,00E+00 3,01E-01 0,00E+00 0,00E+00
GWP kg CO 2 -ekv 3,98E-01 3,09E-01 2,08E+00 1,10E+01 3,24E+01
Climate impact
Parameter Unit B6 B7 C1 C2 C3 C4 D
GWP-IOBC kg CO 2 -ekv 8,99E-05 8,24E-02 3,54E+00 1,12E-03 -3,78E+00
GWP-BCIP kg CO 2 -ekv 0,00E+00 0,00E+00 9,78E+00 0,00E+00 0,00E+00
GWP kg CO 2 -ekv 8,99E-05 8,24E-02 1,33E+01 1,12E-03 -3,78E+00
NEPD-2105-950-EN Fibo wall panels
8/9
Bibliography
DNV GL (2019) PEFC ST 2002:2013. Chain of custody of forest based products. Certificate No. 2018-SKM-
PEFC-274
Ecoinvent v3.5 Swiss Centre of Life Cycle Inventories. www.ecoinvent.ch
EN 15804:2012+A1:2013 Sustainability of construction works - Environmental product declaration - Core rules for the
product category of construction products
GEV (2017) GEV EMICODE license for Fiboseal. Very low emissions: EC1 Plus.
Licence Number: 8477/01.01.05
ISO 14025:2010 Environmental labels and declarations - Type III environmental declarations - Principles and
procedures
ISO 14044:2006 Environmental management - Life cycle assessment - Requirements and guidelines
ISO 21930:2007 Sustainability in building construction - Environmental declaration of building products
NPCR 010:2019 PCR Part B - Product category rules for building boards version 3
NS-EN 16485:2014 Round and sawn timber - Environmental Product Declarations - Product category rules for
wood and wood-based products for use in construction
NS-EN 16449:2014 Wood and wood-based products - Calculation of the biogenic carbon content of wood and
conversion to carbon dioxide
Raadal et al. (2009) Raadal, H. L., Modahl, I. S. & Lyng, K-A. (2009). Klimaregnskap for avfallshåndtering, Fase
I og II. Oppdragsrapport nr 18.09 fra Østfoldforskning.
RISE (2019) Report for emission measurement testresults of Fibo wall panel.
Report reference: 9F007182-01.
Ruttenborg, V. (2019) LCA report for Fibo AS. Report nr. 325049-1 from Norwegian Institute of Wood Technology,
Oslo, Norway.
Statistics Norway (2018a) Table 09469: Net production of district heating by type of heat central, 2017.
Statistics Norway (2018b) Table 04727: District heating balance, 2017.
Statistics Norway (2018c) Table 04730: Consumption of fuel used for gross production of district heating, by type of
energy (GWh), 2017.
Program operator and publisher Phone: +47 97722020
The Norwegian EPD Foundation
Post Box 5250 Majorstuen, 0303 Oslo e-mail: post@epd-norge.no
Norway web www.epd-norge.no
Owner of the declaration Phone: +47 38 34 33 00
Fibo AS Fax
Industriveien 2, NO-4580 Lyngdal e-mail: info@fibo.no
Norway web www.fibo.no
Author of the Life Cycle Assessment Phone: +47 98 85 33 33
Vegard Ruttenborg
Norwegian Institute of Wood Technology e-mail: firmapost@treteknisk.no
P.B. 113 Blindern, NO-0314 Oslo, Norway web www.treteknisk.no
NEPD-2105-950-EN Fibo wall panels
9/9
