ENVIRONMENTAL PRODUCT DECLARATION
as per ISO 14025 and EN 15804+A2
Owner of the Declaration INDURA
Publisher Institut Bauen und Umwelt e.V. (IBU)
Programme holder Institut Bauen und Umwelt e.V. (IBU)
Declaration number EPD-IND-20230364-CBC1-EN
Issue date 20/09/2023
Valid to 19/09/2028
Flanges, weld rings and collars of stainless steel
INDURA
www.ibu-epd.com | https://epd-online.com
General Information
INDURA Flanges, weld rings and collars of stainless steel
Programme holder Owner of the declaration
IBU – Institut Bauen und Umwelt e.V. INDURA
Hegelplatz 1 Grønlandsvej 1
10117 Berlin 7480 Vildbjerg
Germany Denmark
Declaration number Declared product / declared unit
EPD-IND-20230364-CBC1-EN 1 kilogram of flanges, weld rings or collars in stainless steel
This declaration is based on the product category rules: Scope:
Steel pipes for pressure applications, 01/08/2021 A life cycle assessment according to ISO 14040/44 has been conducted
(PCR checked and approved by the SVR) individually for 1 kg (worst-case product) of the three product groups:
• Flanges of stainless steel
• Weld rings of stainless steel
Issue date
• Collars of stainless steel
20/09/2023
Due to the variations in products and production locations, the worst-case
EPD approach has been applied and the highest environmental impacts
Valid to have been declared.
19/09/2028
The materials and metal shaping processes originate from a multitude of
suppliers which INDURA is not in operational control over. The suppliers'
locations are mainly China and India. A conservative average approach
has been applied to make the EPD representative for the suppliers from
different locations, thus Chinese representative data is applied to the
calculation in terms of the energy mix and transport distances. INDURAs
own facility is located in Vildbjerg, Denmark and emissions from that
location are modelled with Danish energy mixes.
The owner of the declaration shall be liable for the underlying information
and evidence; the IBU shall not be liable with respect to manufacturer
Dipl.-Ing. Hans Peters information, life cycle assessment data and evidences.
(Chairman of Institut Bauen und Umwelt e.V.)
The EPD was created according to the specifications of EN 15804+A2. In
the following, the standard will be simplified as EN 15804.
Verification
The standard EN 15804 serves as the core PCR
Independent verification of the declaration and data according to ISO
14025:2011
internally X externally
Florian Pronold Dr.-Ing. Nikolay Minkov,
(Managing Director Institut Bauen und Umwelt e.V.) (Independent verifier)
1 Environmental Product Declaration - INDURA - Flanges, weld rings and collars of stainless steel
Product
• EN10272
Product description/Product definition • EN10028-7
This EPD includes the following products depending on • ASTM A182/A182M
application for oil, gas and water pipe systems: • ASMESA-182/SA182M
• flanges in stainless steel Constructional data
• Weld rings in stainless steel
Name Value Unit
• Collars in stainless steel
Yield strength 205 - 220 N/mm2
The products can come in different dimensions and have
slightly varying shapes such as plate flanges, blind flanges, Tensile strength 520 - 860 N/mm2
neck flanges, weld rings, collars, etc. The declared products are Elongation min. 40 %
classified and traded under the following TARif Intégré
Hardness 140 - 220 HV10
Communautaire (TARIC) code: 7307 21 00 90.
Notched-bar impact value min. 27 - 40 Joule
This EPD specifically excludes the following products:
Ductility min. 40 %
• products in carbon steel and galvanized carbon steel.
• flange gaskets Performance data of the product in accordance with the
• threaded fittings declaration of performance with respect to its essential
• valves. characteristics according to
• EN 1092-1:2018, Flanges and their joints – Circular
For the placing on the market in the European Union/European flanges for pipes, valves, fittings and accessories, PN
Free Trade Association (EU/EFTA) (with the exception of designated – Part 1: Steel flanges.
Switzerland) the following legal provisions apply: 2014/68/EU of
the European Parliament and of the Council of 15 May 2014 on Base materials/Ancillary materials
the harmonization of the laws of the Member States relating to Main material constituents per 1 kg of product in delivery status.
the making available on the market of pressure equipment and
Name Value Unit
the harmonized standards based on these provisions:
Stainless Steel 100 %
• EN 1092-1:2018, Flanges and their joints – Circular
The flanges, weld rings and collars are produced in stainless
flanges for pipes, valves, fittings and accessories, PN
steel, following the material norm EN 10222-5.
designated – Part 1: Steel flanges
The main material constituents in the table above are based on
The CE-marking takes into account the proof of conformity with
the product in delivery status. However, the input of steel is
the respective harmonized standards based on the legal
1.80 kg. Additionally, various packaging materials are also
provisions above. For the application and use the respective
calculated per declared unit. This includes 25*10^-7 kg PVC
national provisions apply.
tape, 0.15 kg cardboard, 0.0011 kg wood EUR pallet, and
Application 0.0027 kg high density polyethylene (HDPE) mesh.
Flanges, weld rings and collars are used to connect different
pipes with each other and can be used both for transporting oils This product/article/at least one partial article contains
and in connection with water. The flanges are usually in the substances listed in the Candidate List of substances of very
form of an annular disc and are attached to the end of a pipe, high concern for Authorisation (published in accordance with
where screws and nuts are used to secure the flange and Article 59(10) of the REACH Regulation) (date: 07-09-2023)
connect the pipes. The different types of flanges include exceeding 0.1 percentage by mass: no.
threaded flanges, blind flanges, welding ring flanges, loose This product/article/at least one partial article contains other
flanges, welding neck flanges, welding neck collars. carcinogenic, mutagenic, reprotoxic (CMR) substances in
categories 1A or 1B which are not on the candidate list,
Technical Data exceeding 0.1 percentage by mass: no.
Flanges, weld rings and collars of stainless steel follow a range Biocide products were added to this construction product or it
of standards in relation to materials, production and technical has been treated with biocide products (this then concerns a
properties, depending on the type of flanges. The following treated product as defined by the (EU) Ordinance on Biocide
standards are relevant for INDURA's products declared in this Products No. 528/2012): no.
EPD:
Reference service life
• EN1092-1
The life cycle of flanges, weld rings and collars is dependent on
• ASME B16.5
the respective structural design, use and maintenance. The use
• DIN2519
phase for steel pipe for oil and gas pipelines is not depicted as
• DIN2576
they involve maintenance-free and generally durable products.
• DIN2642
The reference service life is not declared, as the use phase is
• DIN86044
not included in the scope.
• EN10222-5
LCA: Calculation rules
Declared unit and mass reference
Declared Unit
The declared unit is 1 kg of flanges, weld rings or collars Name Value Unit
stainless steel, where the highest of each LCIA result is Declared unit 1 kg
declared on the final EPD. Conversion factor to metric tonne 1000 -
Density 7900 kg/m3
2 Environmental Product Declaration - INDURA - Flanges, weld rings and collars of stainless steel
System boundary
The product stages (A1 and A3) for flanges, weld rings and and are modelled as inert material landfilling. End-of-life
collars can be seen above. The type of EPD: cradle to gate with treatment of the packaging is not included in the study.
Modules C1–C4 and Module D.
The product stage (modules A1-A3) consists of raw material Benefits and loads beyond the system boundaries (module
extraction and processing (A1) as well as the transport to the D) include the potential benefits from reuse, recycling and
manufacturing location (A2) and activities at the manufacturing recovery potentials that are outside the scope of the study. This
facility (A3). In this study, the processes A1-A3 are all included. would include all the flows leaving the product system having
Wastes and losses of manufacturing processes are included in passed the end-of-waste stage, thereby allowing the use of
the unit processes in which they occur according to the polluter them as a substitution for primary material in another product
pays principle and the modular approach of EN 15804. system. Thus, the system will get credit for recycling the
Practically this means that the metal scrap is modelled so that collected steel. 5 % are considered lost in the sorting process,
its waste processing is included in A3 and credited by reducing thus 95 % of the product is credited in module D.
the input in A1 to the net consumption of steel. However, this
credit cannot exceed the input of secondary metals based on a As the steel scrap from production processes is credited in the
market average. According to the American Iron and Steel A1-A3 modules, only the end-of-life product will be credited in
Institute (American Iron and Steel Institute, 2012) the average module D. The scrap should however first reach functional
recycled content of steel is 36.9 % when it originates from basic equivalence to steel, which requires it to be processed using an
oxygen furnaces. However, for electric arc furnaces, the electric arc furnace (EAF) process. The system is then credited
recycled content is 89.9 %. The sourced materials from Asia with the avoided production of virgin steel produced using the
that INDURA purchases are most likely originating from basic basic oxygen furnace (BOF) process.
oxygen furnaces, but the steel market is constrained (all
available ferrous metal is generally recycled). For this reason, a Geographic Representativeness
total average of the steel recycled content should be applied. It Land or region, in which the declared product system is
is decided that a conservative approach is used in the manufactured, used or handled at the end of the product´s
calculation and the net input of steel is then modelled as lifespan: Denmark
primary (virgin) steel.
Comparability
At the end-of-life stage (module C1-C4), INDURAs products
Basically, a comparison or an evaluation of EPD data is only
are assumed to be manually disassembled from the piping
possible if all the data sets to be compared were created
system in which it has been installed. As a result, no processes
according to EN 15804 and the building context, respectively
have been added to the C1 module. Most customers (>95%)
the product-specific characteristics of performance, are taken
are located in Northern Europe (Scandinavia, Germany and
into account. Furthermore, in order to ensure comparability
Benelux), thus the transportation distances, technology and
between EPDs background databases should be consistent.
waste processing will be modelled accordingly. For the waste
For this declaration, ecoinvent v3.9 has been used.
processing, it is assumed that the product itself will be recycled
as metal. 5 % are considered lost during the recycling process
LCA: Scenarios and additional technical information
Characteristic product properties of biogenic carbon
The biogenic carbon content in the flanges or fittings leaving
the factory gate is 0 %. The biogenic carbon content in the
accompanying packaging is 46 %, as it mainly consists of
cardboard and wood pallet.
3 Environmental Product Declaration - INDURA - Flanges, weld rings and collars of stainless steel
Reuse, recovery and/or recycling potentials (D), relevant
Information on describing the biogenic Carbon Content at scenario information
factory gate Name Value Unit
Name ValueUnit Collection rate 95 %
kg EoL amount 0.590 kg
Biogenic carbon content in product 0
C
5 % losses are assumed in the sorting and recycling system.
Biogenic carbon content in accompanying kg
0.07 This study is a Model EPD where the worst-case scenarios are
packaging C
declared. As a result, module D declares the lowest possible
Note: 1 kg biogenic Carbon is equivalent to 44/12 kg of CO2. recycling credit when compared across the three main product
groups.
Packaging is included and declared in module A3. However, Only the net production of steel scrap is credited for, meaning
since module A5 is not declared in this EPD, the disposal of the that the consumption of secondary steel in A1 is subtracted
packaging material on the construction site is shown below before calculating the credit in module D. The loads associated
including waste amounts and the respective waste scenarios. with the processing of steel scrap must have functional
Per declared unit (1 kg) the following packaging wastes occur: equivalence with steel produced from virgin sources. This is
done through an electric arc furnace process (EAF) process.
• Tape of PVC: 0.00003 kg assumed for landfilling
The amount of steel produced from the collected scrap steel is
• Cardboard box: 0.150 kg assumed for recycling
then credited with the production of steel from virgin sources,
• EUR-pallet of wood: 0.0011 kg assumed for incineration
using a basic oxygen furnace (BOF) process.
• Mesh netting of HDPE: 0.0027 kg assumed for
recycling.
End of life (C1-C4)
Name Value Unit
Collected separately waste type 1 kg
Recycling 0.95 kg
Landfilling 0.05 kg
4 Environmental Product Declaration - INDURA - Flanges, weld rings and collars of stainless steel
LCA: Results
DESCRIPTION OF THE SYSTEM BOUNDARY (X = INCLUDED IN LCA; ND = MODULE OR INDICATOR NOT DECLARED; MNR =
MODULE NOT RELEVANT)
Benefits and
Construction loads beyond
Product stage Use stage End of life stage
process stage the system
boundaries
la ire ta m w a Ry lp p u s tro p s n a rT g n iru tc a fu n a M e h t m o rf tro p s n a rTe tis e h t o t e ta g y lb m e s s A e s U e c n a n e tn ia M ria p e R tn e m e c a lp e R tn e m h s ib ru fe R y g re n e la n o ita re p Oe s u re ta w la n o ita re p Oe s u n o itc u rts n o c -e Dn o itilo m e d tro p s n a rT g n is s e c o rp e ts a W la s o p s iD -e s u e R-y re v o c e R-g n ilc y c e Rla itn e to p
A1 A2 A3 A4 A5 B1 B2 B3 B4 B5 B6 B7 C1 C2 C3 C4 D
X X X MND MND MND MND MNR MNR MNR MND MND X X X X X
RESULTS OF THE LCA - ENVIRONMENTAL IMPACT according to EN 15804+A2: 1 kg flanges, weld rings or collars in stainless
steel
Parameter Unit A1-A3 C1 C2 C3 C4 D
Global Warming Potential total (GWP-total) kg CO 2 eq 9.11E+00 0 4.18E-03 2.21E-02 3.04E-04 -1.58E+00
Global Warming Potential fossil fuels (GWP-fossil) kg CO 2 eq 8.99E+00 0 4.18E-03 2.25E-02 3.04E-04 -1.58E+00
Global Warming Potential biogenic (GWP-biogenic) kg CO 2 eq 1.04E-01 0 3.31E-06 -4.64E-04 1.59E-07 4.36E-03
Global Warming Potential luluc (GWP-luluc) kg CO 2 eq 1.17E-02 0 2.04E-06 2.72E-05 1.83E-07 -2.93E-04
Depletion potential of the stratospheric ozone layer (ODP) kg CFC11 eq 8.83E-08 0 9.16E-11 3.54E-10 8.8E-12 -3.43E-08
Acidification potential of land and water (AP) mol H+ eq 5.06E-02 0 1.95E-05 2.72E-04 2.29E-06 -6.62E-03
Eutrophication potential aquatic freshwater (EP-freshwater) kg P eq 2.93E-03 0 3.01E-07 1.49E-05 2.53E-08 -7.17E-04
Eutrophication potential aquatic marine (EP-marine) kg N eq 9.7E-03 0 7.75E-06 6.07E-05 8.8E-07 -1.5E-03
Eutrophication potential terrestrial (EP-terrestrial) mol N eq 9.7E-02 0 8.29E-05 6.79E-04 9.42E-06 -1.62E-02
Formation potential of tropospheric ozone photochemical oxidants kg NMVOC
3.04E-02 0 2.89E-05 2.01E-04 3.28E-06 -8.49E-03
(POCP) eq
Abiotic depletion potential for non fossil resources (ADPE) kg Sb eq 2.29E-04 0 1.33E-08 1.59E-06 4.28E-10 -1.39E-05
Abiotic depletion potential for fossil resources (ADPF) MJ 1.04E+02 0 6.07E-02 3.07E-01 7.63E-03 -1.47E+01
m3 world eq
Water use (WDP) 2.45E+00 0 3.08E-04 5.46E-03 2.37E-05 -2.65E-01
deprived
RESULTS OF THE LCA - INDICATORS TO DESCRIBE RESOURCE USE according to EN 15804+A2: 1 kg flanges, weld rings or
collars in stainless steel
Parameter Unit A1-A3 C1 C2 C3 C4 D
Renewable primary energy as energy carrier (PERE) MJ 2.38E+01 0 9.53E-04 5.36E-02 6.41E-05 -1.02E+00
Renewable primary energy resources as material utilization
MJ 2.17E+00 0 0 0 0 0
(PERM)
Total use of renewable primary energy resources (PERT) MJ 2.6E+01 0 9.53E-04 5.36E-02 6.41E-05 -1.02E+00
Non renewable primary energy as energy carrier (PENRE) MJ 1.04E+02 0 6.07E-02 3.07E-01 7.63E-03 -1.47E+01
Non renewable primary energy as material utilization (PENRM) MJ 2.86E-01 0 0 0 0 0
Total use of non renewable primary energy resources (PENRT) MJ 1.04E+02 0 6.07E-02 3.07E-01 7.63E-03 -1.47E+01
Use of secondary material (SM) kg 1.13E+00 0 2.7E-05 3.42E-04 1.84E-06 7.82E-01
Use of renewable secondary fuels (RSF) MJ 1.95E-02 0 3.34E-07 1.72E-05 3.94E-08 -1.2E-04
Use of non renewable secondary fuels (NRSF) MJ 0 0 0 0 0 0
Use of net fresh water (FW) m3 6.61E-02 0 7.73E-06 1.56E-04 7.88E-06 -2.87E-03
RESULTS OF THE LCA – WASTE CATEGORIES AND OUTPUT FLOWS according to EN 15804+A2:
1 kg flanges, weld rings or collars in stainless steel
Parameter Unit A1-A3 C1 C2 C3 C4 D
Hazardous waste disposed (HWD) kg 2.76E+00 0 4.08E-05 8.24E-04 3.66E-06 -2.33E-01
Non hazardous waste disposed (NHWD) kg 1.35E+01 0 1.27E-03 5.85E-02 1.1E-04 -2.82E+00
Radioactive waste disposed (RWD) kg 4.72E-05 0 4.97E-09 1.66E-07 3.2E-10 2.49E-06
Components for re-use (CRU) kg 0 0 0 0 0 0
Materials for recycling (MFR) kg 5.14E-01 0 4.57E-07 1E+00 3.42E-08 -9.68E-05
Materials for energy recovery (MER) kg 1.38E-04 0 2.82E-09 4.63E-08 1.23E-10 -8.47E-06
Exported electrical energy (EEE) MJ 3.47E-02 0 1E-05 3.75E-04 4.19E-07 1.11E-02
Exported thermal energy (EET) MJ 1.64E-01 0 2.37E-05 5.76E-05 2.61E-07 -1.37E-02
RESULTS OF THE LCA – additional impact categories according to EN 15804+A2-optional:
1 kg flanges, weld rings or collars in stainless steel
Parameter Unit A1-A3 C1 C2 C3 C4 D
Disease
Incidence of disease due to PM emissions (PM) 7.22E-07 0 4.11E-10 3.65E-09 5.01E-11 -1.09E-07
incidence
Human exposure efficiency relative to U235 (IR) kBq U235 eq 6.09E-01 0 8.34E-05 2.74E-03 4.8E-06 5.38E-02
5 Environmental Product Declaration - INDURA - Flanges, weld rings and collars of stainless steel
Comparative toxic unit for ecosystems (ETP-fw) CTUe 4.54E+01 0 2.95E-02 2.37E-01 3.54E-03 -2.64E+00
Comparative toxic unit for humans (carcinogenic) (HTP-c) CTUh 2E-07 0 2.33E-12 4.19E-11 1.37E-13 9.95E-09
Comparative toxic unit for humans (noncarcinogenic) (HTP-nc) CTUh 2.23E-07 0 4.71E-11 1.75E-09 1.64E-12 -1.17E-08
Soil quality index (SQP) SQP 6.17E+01 0 4.53E-02 5.87E-01 1.5E-02 -4.63E+00
Disclaimer 1 – for the indicator 'Potential Human exposure efficiency relative to U235'. This impact category deals mainly with the
eventual impact of low-dose ionizing radiation on human health of the nuclear fuel cycle. It does not consider effects due to possible
nuclear accidents, occupational exposure or radioactive waste disposal in underground facilities. Potential ionizing radiation from the
soil, radon and from some construction materials is also not measured by this indicator.
Disclaimer 2 – for the indicators 'abiotic depletion potential for non-fossil resources', 'abiotic depletion potential for fossil resources',
'water (user) deprivation potential, deprivation-weighted water consumption', 'potential comparative toxic unit for ecosystems', 'potential
comparative toxic unit for humans – cancerogenic', 'Potential comparative toxic unit for humans - not cancerogenic', 'potential soil
quality index'. The results of this environmental impact indicator shall be used with care as the uncertainties on these results are high
as there is limited experience with the indicator.
References
Standards Steel forgings for pressure purposes-Part 5: Martensitic,
ASTM A182/A182M austenitic and austenitic - ferritic stainless steels
Specification for forged or rolled alloy and stainless steel pipe EN 10272
flanges, forged fittings, and valves and parts for high Stainless steel bars for pressure purposes
temperature service ISO 14025
ASME B16.5 EN ISO 14025:2011, Environmental labels and declarations —
B16.5 - 2020, Pipe Flanges and Flanged Fittings: NPS 1/2 Type III environmental declarations — Principles and
through NPS 24, Metric/Inch Standard. procedures.
ASMESA-182/SA182M Further references
Specification for forged or rolled alloy and stainless steel pipe American Iron and Steel Institute. (2012).
flanges, forged fittings, and valves and parts for high CSSBI. Steel Takes LEED® with Recycled Content. From
temperature service https://cssbi.ca/ [access on 10-12-2022]
DIN 2519 Candidate List of Substances of Very High Concern
German norm for steel flanges https://echa.europa.eu/candidate-list-table [access on 12-06-
DIN 2576 23]
German norm for plate flanges EcoInvent 3.9
DIN 2642 EcoInvent database version 3.9, cut-off, EN15804 model. LCIA
German norm for loose plate flanges methodology EF v3.1 EN15804. Wernet, G., Bauer, C.,
DIN 86044 Steubing, B., Reinhard, J., Moreno-Ruiz, E., and Weidema, B.,
German norm for plate flanges 2016. The ecoinvent database version 3 (part I): overview and
Documents provided by the Institut Bauen und Umwelt methodology. The International Journal of Life Cycle
e.V.: Assessment, [online] 21(9), pp.1218–1230. Available at:
Product Category Rules for Building-Related Products and [Accessed 10-12-2022].
Services: Part A: Calculation Rules for the Life Cycle IBU 2021
Assessment and Requirements on the Project Report according Institut Bauen und Umwelt e.V.: General Instructions for the
to EN 15804+A2:2019 version 1.3 EPD programme of Institut Bauen und Umwelt e.V., Version
Product Category Rules Part B: Requirements on the EPD for 2.0, Berlin: Institut Bauen und Umwelt e.V., 2021 www.ibu-
Steel pipes for pressure applications 01/08/2021 (version 1). epd.com
EN 15804 INDURA
EN 15804+A2:2019, Sustainability of construction works — https://www.indura.com/products [access on 10-12-22]
Environmental Product Declarations — Core rules for the Ordinance on Biocide Products No. 528/2012
product category of construction products. Regulation (EU) No 528/2012 of the European Parliament and
EN ISO 14040/44 of the Council of 22 May 2012 concerning the making available
EN ISO 14040:2006, Environmental management – Life cycle on the market and use of biocidal products Text with EEA
assessment - Principles and framework; English version EN relevance.
ISO 14040:2006 EN ISO 14044:2006, Environment http://data.europa.eu/eli/reg/2012/528/oj [access on 12-06-23]
Management – Life Cycle Assessment – Requirements and SimaPro 2023
Instructions; English version EN ISO 14044:2006. LCA Software; PRé Sustainability, Version 9.5
EN 1092-1 TARIC
EN 1092-1:2018, TARIC, the integrated Tariff of the European Union, is a
Flanges and their joints – Circular flanges for pipes, valves, multilingual database integrating all measures relating to EU
fittings and accessories, PN designated – Part 1: Steel flanges. customs tariff, commercial and agricultural legislation. Link to
EN 10028-7 database: https://ec.europa.eu/taxation_customs/dds2/taric/
Flat products made of steels for pressure purposes - Part 7: [access on 12-06-23]
Stainless steels
EN10222-5
6 Environmental Product Declaration - INDURA - Flanges, weld rings and collars of stainless steel
Publisher
Institut Bauen und Umwelt e.V. +49 (0)30 3087748- 0
Hegelplatz 1 info@ibu-epd.com
10117 Berlin www.ibu-epd.com
Germany
Programme holder
Institut Bauen und Umwelt e.V. +49 (0)30 3087748- 0
Hegelplatz 1 info@ibu-epd.com
10117 Berlin www.ibu-epd.com
Germany
Author of the Life Cycle Assessment
Viegand Maagøe +4533349000
Nørre Farigmagsgade 37 info@viegandmaagoe.dk
1364 Copenhagen www.viegandmaagoe.dk/en
Denmark
Owner of the Declaration
INDURA +45 97133244
Grønlandsvej 1 salg@indura.dk
7480 Vildbjerg www.indura.dk/
Denmark
7 Environmental Product Declaration - INDURA - Flanges, weld rings and collars of stainless steel
