ENVIRONMENTAL PRODUCT DECLARATION
as per ISO 14025 and EN 15804+A2
Owner of the Declaration Magnetic Autocontrol GmbH
Publisher Institut Bauen und Umwelt e.V. (IBU)
Programme holder Institut Bauen und Umwelt e.V. (IBU)
Declaration number EPD-MAG-20230361-CCI1-EN
Issue date 16.01.2024
Valid to 15.01.2029
FlowMotion® mWing
Magnetic Autocontrol GmbH
www.ibu-epd.com | https://epd-online.com
General Information
Magnetic Autocontrol GmbH FlowMotion® mWing
Programme holder Owner of the declaration
IBU – Institut Bauen und Umwelt e.V. Magnetic Autocontrol GmbH
Hegelplatz 1 Grienmatt 20
10117 Berlin 79650 Schopfheim
Germany Germany
Declaration number Declared product / declared unit
EPD-MAG-20230361-CCI1-EN 1 piece of FlowMotion® mWing speed gate (standard height)
This declaration is based on the product category rules: Scope:
Electronic and physical Access Control Systems, 01.08.2021 The EPD refers to FlowMotion® mWing speed gate (Product dimensions:
(PCR checked and approved by the SVR) 1300 x 1050 x 180 mm; glass door standard height: 888 mm)
manufactured by Magnetic Autocontrol GmbH. The production site for the
product is situated in Schopfheim, Germany. The pre-products are
Issue date supplied from Germany, Italy, Bulgaria, China, Iceland, Tunisia, Indonesia
and Great Britain.
16.01.2024
The LCA results declared in the EPD are based on the data collected in
2022 and cover the entire life cycle of FlowMotion® mWing speed gate
Valid to
(standard height).
15.01.2029
The owner of the declaration shall be liable for the underlying information
and evidence; the IBU shall not be liable with respect to manufacturer
information, life cycle assessment data and evidences.
The EPD was created according to the specifications of EN 15804+A2. In
the following, the standard will be simplified as EN 15804.
Verification
The standard EN 15804 serves as the core PCR
Independent verification of the declaration and data according to ISO
14025:2011
Dipl.-Ing. Hans Peters
(Chairman of Institut Bauen und Umwelt e.V.) internally X externally
Florian Pronold Dr.-Ing. Nikolay Minkov,
(Managing Director Institut Bauen und Umwelt e.V.) (Independent verifier)
1 Environmental Product Declaration - Magnetic Autocontrol GmbH - FlowMotion® mWing
Product
for drives for gates, doors and windows
Product description/Product definition • EN 60034-1 Duty cycle S1 (continuous operation),
The FlowMotion® mWing is designed for the control of persons 100%
entering or leaving an area with restricted access. The • EN 13849-1 Performance Level d
FlowMotion® mWing speed gate is intended for the passage of • DIN EN 61000-6-2: 2005 and Amendment:2011
persons safely, speedily and without any help. Different security Electromagnetic Compatibility (EMC)
levels are possible, mechanical locking and comprehensive • DIN EN 61000-6-3:2007 and A1:2011 Electromagnetic
monitoring of the access area. Compatibility (EMC)
• Enclosure protection rating: IP54 (according EN 60529)
Magnetic drive technology complies with current norms and • Blocking element: single-layer safety glass according
standards, including DIN EN 17352. To ensure user safety at all EN 12150-1, laminated glass according EN ISO 12543-
times without the need for complex and expensive monitoring 1 and EN ISO 12543-2 or acrylic glass EN ISO 179-1
equipment, the Magnetic Safety Drive System (MSDS®) • Escape and rescue route approval:
complies with an innovative low-energy concept. The According to EltVTR (Directive on electrical locking
interaction of the drive motor, power supply and control system systems for doors in escape routes). This is currently
ensures that only a limited amount of energy can be fed into the still the valid standard for Germany.
system at any time. This means that all Momentum family locks • DIN EN 13637 (locks and building hardware -
with MSDS are safe to use at all times. electrically controlled escape door systems for doors in
escape routes - requirements and test methods).
The housing is made out of mDure® (Polyurethane) with a wide • Resistant against corrosion, UV light, detergents and
range of colour options. It is highly resistant to impacts, disinfectants. UL tested according to UL0746C f1
scratches and abrasion. It can cushion mechanical effects (yellow card E 83364)
without suffering any lasting deformation. The material is • Fire behavior: tested according to UL-94 V0 and UL
extremely durable and chemically resistant – against 0746C
disinfectants and detergents, as well as against aggressive
chemicals, UV radiation and corrosion. It is free of pollutants Application
and can be recycled, disposed of as household waste, or burnt The product can be used at the following locations:
without polluting the environment.
• Office and administrative buildings
• Ministries and government building
The product consists of a stainless steel base frame and plate.
• Banks and financial institutions
The wings are made of glass. The side panels of the housing
• Industrial buildings
are attached to the frame without any visible connecting
• Schools and universities
elements and thus create the impression of seamless
• Sportive areas
construction.
• Indoor and outdoor use
User guidance: Technical Data
• Frame-edge illumination is integrated and light elements The product is delivered in two separate modules, each packed
offer flexible use to show operational readiness, the individually. The details of each module are given below:
direction of passage or the validity of access 1. Module 1:
authorization Name: FMWI_AL, mWing A-Modul
• The white floor illumination simplifies orientation in the Weight without packaging: 75 kg
entrance area for visitors.
• The passage direction indicator in the front face plate 2. Module 2:
shows visitors if the passage is open to them and Name: FMWI_BL, mWing B-Modul
whether they have valid access authorization. Weight without packaging: 79 kg
Information on Packaging:
Unobstructed escape routes: Mainly corrugated board (13.2 kg) and wooden pallets (22.2 kg)
mWing allows free passage in the case of a power outage or an are used for packaging of the products. The other packaging
alarm signal. The wing doors allow the setting up of particularly material includes steel screws, steel sheet and plastic film and
wide, officially approved escape routes. the total packaging weight is 35.8 kg. Total weight of module A
and module B including packaging is 190.5 kg.
For the placing on the market in the European Union/European
Free Trade Association (EU/EFTA) (with the exception of Constructional data
Switzerland) the following legal provisions apply:
Directives:
• Machinery Directive 2006/42/EC
• Electromagnetic Compatibility Directive 2014/30/EU
• ROHS2 Directive 2011/65/EU
Norms and standards:
• EN17352:2022 Power operated pedestrian entrance
control equipment - Safety in use - Requirements and
test methods
• EN 60335-2-103 Household and similar electrical
appliances - Safety - Part 2-103: Particular requirements
2 Environmental Product Declaration - Magnetic Autocontrol GmbH - FlowMotion® mWing
Name Value Unit • EN 60034-1 Duty cycle S1 (continuous operation),
100%
Power supply /supply voltage 100 to 240 V AC ±
V • EN 13849-1 Performance Level d
(minimum) 10 %, 50 to 60 Hz
• DIN EN 61000-6-2: 2005 and Amendment:2011
Current Requirements 1 - 2.4 A
Electromagnetic Compatibility (EMC)
Operating Temprature -30 to +55 °C
• DIN EN 61000-6-3:2007 and A1:2011 Electromagnetic
Power consumption "Operating Compatibility (EMC)
35 W
without illumination and locking unit" • Enclosure protection rating: IP54 (according EN 60529)
Power consumption "Operating with • Blocking element: single-layer safety glass according
87 W
illumination" EN 12150-1, laminated glass according EN ISO 12543-
Power consumption "Operating with 1 and EN ISO 12543-2 or acrylic glass EN ISO 179-1
illumination and locking unit" 107 W • Escape and rescue route approval: According to EltVTR
(Directive on electrical locking systems for doors in
Power consumption "Standby without
20 W escape routes). This is currently still the valid standard
illumination and locking unit"
for Germany.
Power consumption "Standby with
72 W • DIN EN 13637 (locks and building hardware -
Illumination
electrically controlled escape door systems for doors in
Power consumption "Standby with escape routes - requirements and test methods
102 W
illumination and locking unit"
Base materials/Ancillary materials
Ambient Temperature -30 to +55 °C
The weight of the product without packaging is 154 kg. The
Height (Dimension) 1.05 m
material composition is given in the following table:
Width (Dimension) 0.18 m
Name Value Unit
Length (Dimension) 1.3 m
Glass 32 %
IP rating IP54
Plastics 30 %
Applicability Indoor and outdoor
Steel 28 %
Product not harmonised in accordance with CPR bit in
Aluminium 2 %
accordance with other provisions for harmonisation of the EU:
Others (cables, magnets, electronics etc.) 8 %
• Machinery Directive 2006/42/EC This product/article/at least one partial article contains
• Electromagnetic Compatibility Directive 2014/30/EU substances listed in the candidate list (date: 28/06/2023)
• ROHS2 Directive 2011/65/EU exceeding 0.1 percentage by mass: no
• EN17352:2022 Power operated pedestrian entrance
Reference service life
control equipment - Safety in use - Requirements and
As an RSL according to ISO 15686 cannot be declared, the
test methods
service life according to the "Bewertungssystem Nachhaltiges
• EN 60335-2-103 Household and similar electrical
Bauen (BNB)" is 20 years, which corresponds to 14.6 million
appliances - Safety - Part 2-103: Particular requirements
closing cycles.
for drives for gates, doors and windows
LCA: Calculation rules
• The product has no direct emissions (B1) and is
Declared Unit designed so that no maintenance is required (B2) or
The declared functional unit is to provide 14,6 Million closing parts need to be replaced (B4). Furthermore, no
cycles during a reference lifetime of 20 years i.e. equivalent to 1 standard repairs (B3) or refurbishments (B5) are fore-
unit of FlowMotion® mWing speed gate (Product dimensions: seen. The use of the product does not require water
1300 x 1050 x 180 mm; glass door standard height: 888 mm). consumption (B7) but requires electricity (B6)
Declared unit throughout its use stage.
• Module C1 includes manual disassembly of the product
Name Value Unit
and C2 includes transportation of the waste to treatment
Declared unit 1 pce.
site. Module C3 and C4 include emissions of processing
Mass reference 190.5 kg/pce waste through a shredder and waste land filling and the
final disposal of waste.
• Module D comprises the recycling of metals and gives
System boundary the recycling potentials as well as potential benefits from
Type of EPD: cradle to grave energy substitution.
Geographic Representativeness
The system boundary of the EPD follows the modular structure
Land or region, in which the declared product system is
defined by EN 15804.
manufactured, used or handled at the end of the product´s
• Modules A1 to A3 include the provision and processing
lifespan: Europe
of raw materials and pre-products, the transport to the
manufacturer's production site and the production of the
mWing product. Comparability
• Module A4 includes the transportation of the product to Basically, a comparison or an evaluation of EPD data is only
the installation site. Module A5 covers the manual possible if all the data sets to be compared were created
installation of the product (negligible impact) and according to EN 15804 and the building context, respectively
treatment and disposal of packaging material. the product-specific characteristics of performance, are taken
into account. LCA is conducted using LCA for expert software
3 Environmental Product Declaration - Magnetic Autocontrol GmbH - FlowMotion® mWing
along with Managed Lifecycle Content (MLC) (previously known as Gabi) MLC Modelling Database CUP Version 2022.2.
LCA: Scenarios and additional technical information
Service life is declared by the manufacturer and is valid under
Characteristic product properties of biogenic carbon ambient conditions stated under construction data.
The calculation of the biogenic carbon content is based on the
Reference service life
technical consideration, that one kilogram of corrugated board
(paper) consists of 43% biogenic carbon by mass and one Name Value Unit
kilogram of pallet with 40% water content consists of 36% of Life Span according to the manufacturer 20 a
biogenic carbon. The product consists of 0.0044 kg of
corrugated board in the form of paper labelling. Packaging Operational energy use (B6)
consists of 13.2 kg of corrugated board and 22.2 kg of wooden Based on the parameters listed below, the total energy
pallets per piece of mWing module. consumption for 14.6 million cycles in 20 years is 3624 kWh.
Name Value Unit
Note: 1 kg of biogenic carbon is equivalent to 44/12 kg of CO .
2 Electricity consumption (Operating mode) 35 W
Information on describing the biogenic Carbon Content at Electricity consumption (Normal Standby Current) 20 W
factory gate Cycle duration 2 s
Name Value Unit Closing cycles per day 2000 times
kg Operating mode per day 1,1 hours
Biogenic carbon content in product 0.0019
C
Standby mode per day 22,9 hours
Biogenic carbon content in accompanying kg
13.7
packaging C End of life (C1-C4)
The collection rate of the product is 100% and the waste
collected is processed at the end of life under the scenarios
The following technical scenario information is required for
defined in the table below.
the declared modules:
Name Value Unit
Collected separately waste type waste type 155 kg
Transport to the building site (A4)
Table shows the average distance between the production site Recycling 54.25 kg
and the European installation site. The product is transported Energy recovery 48.05 kg
via Truck. Landfilling 52.7 kg
Name Value Unit
Reuse, recovery and/or recycling potentials (D), relevant
Transport distance 677 km
scenario information
Capacity utilisation (including empty runs) 61 %
Product is not intended for re-used. Assumed collection rate of
100%. Net credits are received for the energy recovery after
Installation into the building (A5)
incineration and secondary material production after recycling
mWing module is installed manually on the site which requires
metals, plastics and electronics.
negligible material and energy inputs. A5 further includes the
treatment of packaging waste. The packaging waste consists of
a wooden pallet, plastic wrap and metals parts (e.g. screws). Name Value Unit
Name ValueUnit Note: Modules B1-B5, B7 and C1 are zero have negligible
Output substances following waste treatment on material and energy inputs as described under the the section
site (packaging) 35.8 kg "system boundary".
4 Environmental Product Declaration - Magnetic Autocontrol GmbH - FlowMotion® mWing
LCA: Results
The LCA results provided are provided for 1 unit of FlowMotion® mWing speed gate (standard height) with a service life of 20 years
committing 14.6 million closing cycles.
Note: The impact of the product for the modules B1-B5, B7 and C1 are zero under the conditions described in the section "system
boundary".
DESCRIPTION OF THE SYSTEM BOUNDARY (X = INCLUDED IN LCA; MND = MODULE OR INDICATOR NOT DECLARED; MNR
= MODULE NOT RELEVANT)
Benefits and
Construction loads beyond
Product stage Use stage End of life stage
process stage the system
boundaries
la ire ta m w a Ry lp p u s tro p s n a rT g n iru tc a fu n a M e h t m o rf tro p s n a rTe tis e h t o t e ta g y lb m e s s A e s U e c n a n e tn ia M ria p e R tn e m e c a lp e R tn e m h s ib ru fe R y g re n e la n o ita re p Oe s u re ta w la n o ita re p Oe s u n o itc u rts n o c -e Dn o itilo m e d tro p s n a rT g n is s e c o rp e ts a W la s o p s iD -e s u e R-y re v o c e R-g n ilc y c e Rla itn e to p
A1 A2 A3 A4 A5 B1 B2 B3 B4 B5 B6 B7 C1 C2 C3 C4 D
X X X X X X X X X X X X X X X X X
RESULTS OF THE LCA - ENVIRONMENTAL IMPACT according to EN 15804+A2: 1 piece FlowMotion® mWing speed gate
(standard height)
Parameter Unit A1 A2 A3 A4 A5 B1 B2 B3 B4 B5 B6 B7 C1 C2 C3 C4 D
GWP-total kg CO 2 6.59E 5.31E 8.44E 9.85E 3.7E+01 0 0 0 0 0 1.35E 0 0 5.91E 1.2E+027.63E-01 -1.89E
eq +02 +00 +02 +00 +03 +00 +02
GWP-fossil kg CO 2 6.58E 5.41E 8.97E 1E+01 1.14E 0 0 0 0 0 1.34E 0 0 6.02E 1.2E+027.84E-01 -1.89E
eq +02 +00 +02 +00 +03 +00 +02
GWP- kg CO 2 1.17E 0 -5.31E 0 3.59E 0 0 0 0 0 1.21E 0 0 0 1.59E- -2.28E- -3.24E-
biogenic eq +00 +01 +01 +01 01 02 01
GWP-luluc kg CO 2 2.01E- 3.6E-02 1.07E- 6.68E- 1E-04 0 0 0 0 0 2.83E- 0 0 4E-02 7.82E- 1.43E-03 -4.69E-
eq 01 01 02 01 03 02
kg CFC11 5.86E- 5.24E- 9.73E- 3.89E- 1.96E- 5.84E- 2.88E-
ODP 1.3E-09 0 0 0 0 0 0 0 1.86E-12 -4E-10
eq 09 13 13 12 08 13 10
2.97E 8.26E- 2.04E- 5.78E- 2.94E 1.23E- 5.45E- -6.11E-
AP mol H+ eq 1.1E-02 0 0 0 0 0 0 0 5.48E-03
+00 01 02 03 +00 02 02 01
EP- 1.33E- 1.91E- 1.39E- 3.54E- 9.26E- 3.91E- 2.12E- 5.99E- -1.56E-
kg P eq 0 0 0 0 0 0 0 1.32E-06
freshwater 03 05 03 05 07 03 05 05 04
5.46E- 4.57E- 3.18E- 8.48E- 1.91E- 6.59E- 5.09E- 1.17E- -1.07E-
EP-marine kg N eq 0 0 0 0 0 0 0 1.4E-03
01 03 01 03 03 01 03 02 01
5.95E 5.21E- 3.42E 9.66E- 6.92E 5.79E- 1.64E- -1.16E
EP-terrestrial mol N eq 2.7E-02 0 0 0 0 0 0 0 1.54E-02
+00 02 +00 02 +00 02 01 +00
kg
1.69E 9.82E- 8.73E- 1.82E- 5.21E- 1.78E 1.09E- 4.61E- -3.48E-
POCP NMVOC 0 0 0 0 0 0 0 4.26E-03
+00 03 01 02 03 +00 02 02 01
eq
1.47E- 5.38E- 6.15E- 9.99E- 3.65E- 5.99E- 7.48E- -6.15E-
ADPE kg Sb eq 9.5E-08 0 0 0 0 0 0 0 8.05E-08
02 07 05 07 04 07 06 03
9.86E 7.01E 1.39E 8.76E 2.43E 2.61E 1.03E -2.14E
ADPF MJ 1.3E+02 0 0 0 0 0 0 0 7.8E+01
+03 +01 +04 +00 +04 +02 +01 +03
m3 world
2.29E 5.97E- 5.79E 1.11E- 3.88E 3.05E 6.65E- 6.72E -7.42E
WDP eq 0 0 0 0 0 0 0 8.77E-02
+02 02 +00 01 +00 +02 02 +00 +00
deprived
GWP = Global warming potential; ODP = Depletion potential of the stratospheric ozone layer; AP = Acidification potential of land and water; EP =
Eutrophication potential; POCP = Formation potential of tropospheric ozone photochemical oxidants; ADPE = Abiotic depletion potential for non-fossil
resources; ADPF = Abiotic depletion potential for fossil resources; WDP = Water (user) deprivation potential)
RESULTS OF THE LCA - INDICATORS TO DESCRIBE RESOURCE USE according to EN 15804+A2: 1 piece FlowMotion®
mWing speed gate (standard height)
Parameter Unit A1 A2 A3 A4 A5 B1 B2 B3 B4 B5 B6 B7 C1 C2 C3 C4 D
1.51E 4.86E 1.43E 9.01E 1.35E 5.41E 1.26E 1.54E -3.73E
PERE MJ 4.8E+02 0 0 0 0 0 0 0
+03 +00 +03 +00 +04 +00 +02 +00 +02
7.92E- 4.77E -4.77E 7.92E-
PERM MJ 0 0 0 0 0 0 0 0 0 0 0 0 0
02 +02 +02 02
1.51E 4.86E 9.51E 9.01E 2.31E 1.35E 5.41E 1.26E 1.54E -3.73E
PERT MJ 0 0 0 0 0 0 0
+03 +00 +02 +00 +00 +04 +00 +02 +00 +02
8.28E 7.04E 1.39E 1.31E 1.69E 2.43E 7.83E -1.33E 1.03E -2.15E
PENRE MJ 0 0 0 0 0 0 0
+03 +01 +04 +02 +01 +04 +01 +03 +01 +03
1.59E 8.08E -8.08E 1.59E
PENRM MJ 0 0 0 0 0 0 0 0 0 0 0 0 0
+03 +00 +00 +03
PENRT MJ 9.87E 7.04E 1.39E 1.31E 8.77E 0 0 0 0 0 2.43E 0 0 7.83E 2.61E 1.03E -2.15E
5 Environmental Product Declaration - Magnetic Autocontrol GmbH - FlowMotion® mWing
+03 +01 +04 +02 +00 +04 +01 +02 +01 +03
3.65E- 1.07E
SM kg 0 0 0 0 0 0 0 0 0 0 0 0 0 0 0
03 +01
RSF MJ 0 0 0 0 0 0 0 0 0 0 0 0 0 0 0 0 0
NRSF MJ 0 0 0 0 0 0 0 0 0 0 0 0 0 0 0 0 0
6.68E 5.61E- 1.27E 1.04E- 9.14E- 1.29E 6.25E- 2.29E- 2.65E- -6.07E-
FW m3 0 0 0 0 0 0 0
+00 03 +00 02 02 +01 03 01 03 01
PERE = Use of renewable primary energy excluding renewable primary energy resources used as raw materials; PERM = Use of renewable primary
energy resources used as raw materials; PERT = Total use of renewable primary energy resources; PENRE = Use of non-renewable primary energy
excluding non-renewable primary energy resources used as raw materials; PENRM = Use of non-renewable primary energy resources used as raw
materials; PENRT = Total use of non-renewable primary energy resources; SM = Use of secondary material; RSF = Use of renewable secondary fuels;
NRSF = Use of non-renewable secondary fuels; FW = Use of net fresh water
RESULTS OF THE LCA – WASTE CATEGORIES AND OUTPUT FLOWS according to EN 15804+A2:
1 piece FlowMotion® mWing speed gate (standard height)
Parameter Unit A1 A2 A3 A4 A5 B1 B2 B3 B4 B5 B6 B7 C1 C2 C3 C4 D
3.29E- 3.72E- 5.83E- 6.91E- 8.52E- 4.14E- -1.32E-
HWD kg 0 0 0 0 0 2.1E-06 0 0 7.1E-08 5.6E-10
05 10 06 10 10 10 07
4.27E 1.15E- 5.93E 2.13E- 3.87E- 1.83E 1.28E- 8.28E 5.17E -8.79E
NHWD kg 0 0 0 0 0 0 0
+01 02 +00 02 01 +01 02 +00 +01 +00
1.66E- 1.31E- 2.42E- 5.16E- 3.88E 1.45E- 1.12E- 1.18E-
RWD kg 6.3E-01 0 0 0 0 0 0 0 -9E-02
01 04 04 04 +00 04 02 04
CRU kg 0 0 0 0 0 0 0 0 0 0 0 0 0 0 0 0 0
4.78E
MFR kg 0 0 0 0 1.4E-01 0 0 0 0 0 0 0 0 0 0 0
+01
2.19E
MER kg 0 0 0 0 0 0 0 0 0 0 0 0 0 0 0 0
+01
5.37E
EEE MJ 0 0 0 0 0 0 0 0 0 0 0 0 0 1.5E+02 0 0
+01
9.65E 3.47E
EET MJ 0 0 0 0 0 0 0 0 0 0 0 0 0 0 0
+01 +02
HWD = Hazardous waste disposed; NHWD = Non-hazardous waste disposed; RWD = Radioactive waste disposed; CRU = Components for re-use;
MFR = Materials for recycling; MER = Materials for energy recovery; EEE = Exported electrical energy; EET = Exported thermal energy
RESULTS OF THE LCA – additional impact categories according to EN 15804+A2-optional:
1 piece FlowMotion® mWing speed gate (standard height)
Parameter Unit A1 A2 A3 A4 A5 B1 B2 B3 B4 B5 B6 B7 C1 C2 C3 C4 D
Disease
PM ND ND ND ND ND ND ND ND ND ND ND ND ND ND ND ND ND
incidence
kBq U235
IR ND ND ND ND ND ND ND ND ND ND ND ND ND ND ND ND ND
eq
ETP-fw CTUe ND ND ND ND ND ND ND ND ND ND ND ND ND ND ND ND ND
HTP-c CTUh ND ND ND ND ND ND ND ND ND ND ND ND ND ND ND ND ND
HTP-nc CTUh ND ND ND ND ND ND ND ND ND ND ND ND ND ND ND ND ND
SQP SQP ND ND ND ND ND ND ND ND ND ND ND ND ND ND ND ND ND
PM = Potential incidence of disease due to PM emissions; IR = Potential Human exposure efficiency relative to U235; ETP-fw = Potential comparative
Toxic Unit for ecosystems; HTP-c = Potential comparative Toxic Unit for humans (cancerogenic); HTP-nc = Potential comparative Toxic Unit for humans
(not cancerogenic); SQP = Potential soil quality index
The LCA results of "1 piece FlowMotion® mWing speed gate (standard height)" are not declared for additional impact categories
according to EN 15804+A2: optional as the uncertainties in these indicators are high.
Disclaimer 1 – for the indicator 'Potential Human exposure efficiency relative to U235'. This impact category deals mainly with the
eventual impact of low-dose ionizing radiation on human health of the nuclear fuel cycle. It does not consider effects due to possible
nuclear accidents, occupational exposure or radioactive waste disposal in underground facilities. Potential ionizing radiation from the
soil, radon and from some construction materials is also not measured by this indicator.
Disclaimer 2 – for the indicators 'abiotic depletion potential for non-fossil resources', 'abiotic depletion potential for fossil resources','
water (user) deprivation potential, deprivation-weighted water consumption', 'potential comparative toxic unit for ecosystems',' potential
comparative toxic unit for humans – cancerogenic', 'Potential comparative toxic unit for humans - not cancerogenic',' potential soil
quality index'. The results of this environmental impact indicator shall be used with care as the uncertainties on these results are high
as there is limited experience with the indicator.
6 Environmental Product Declaration - Magnetic Autocontrol GmbH - FlowMotion® mWing
References
Directives residential, commercial and light-industrial environments.
Machinery Directive 2006/42/EC EN 60529
Machinery Directive 2006/42/EC on machinery, and amending DIN EN 60529:2014-09, Degrees of protection provided by
Directive 95/16/EC (recast) enclosures (IP Code) (IEC 60529:1989 + A1:1999 + A2:2013)
Electromagnetic Compatibility Directive 2014/30/EU EN 12150-1
Electromagnetic Compatibility Directive 2014/30/EU on the EN 12150-1:2020-07, Glass in building - Thermally toughened
harmonization of the laws of the Member States relating to soda lime silicate safety glass - Part 1: Definition and
electromagnetic compatibility (recast) description
ROHS2 Directive 2011/65/EU EN ISO 12543- 1
Directive 2011/65/EU on the restriction of the use of certain EN ISO 12543-1:2011-12, Glass in building - Laminated glass
hazardous substances in electrical and electronic equipment and laminated safety glass - Part 1: Definitions and description
(recast) of component parts (ISO 12543-1:2011)
Standards and Norms: EN ISO 12543-2
EN ISO 12543-2:2022-03, Glass in building - Laminated glass
EN 15804 and laminated safety glass - Part 2: Laminated safety glass
EN 15804:2012+A2:2019+AC:2021, Sustainability of (ISO 12543-2:2021)
construction works - Environmental Product Declarations - Core
rules for the product category of construction products. EN ISO 179-1
EN ISO 179-1:2010-11, Plastics - Determination of Charpy
EN ISO 14040 impact properties - Part 1: Non-instrumented impact test (ISO
EN ISO 14044:2006-10 Environmental management - Life 179-1:2010)
cycle assessment - Requirements and guidelines
DIN EN 13637
EN ISO 14044: http DIN EN 13637:2015-12, Building hardware - Electrically
EN ISO 14044:2006-10 Environmental management - Life controlled exit systems for use on escape routes -
cycle assessment - Requirements and guidelines Requirements and test methods
EN17352:2022 ISO 14025
EN17352:2022 Power operated pedestrian entrance control EN ISO 14025:2011, Environmental labels and declarations —
equipment - Safety in use - Requirements and test methods Type III environmental declarations — Principles and
procedures.
EN 60335-2-103
EN 60335-2-103 Household and similar electrical appliances - REACH
Safety - Part 2-103: Particular requirements for drives for gates, REACH Regulation (EC) No 1907/2006 concerning the
doors and windows (IEC 60335-2-103:2006, modified + Registration, Evaluation, Authorization and Restriction of
A1:2010, modified) Chemicals (REACH)
EN 60034-1 UL0746C
EN 60034-1 VDE 0530-1:2011-02, Rotating electrical UL 746C:2018-02-05, Polymeric materials - Use in electrical
machines, Part 1: Rating and performance (IEC 60034-1:2010, equipment evaluations
modified)
UL 94
EN ISO 13849-1:2016-06 Standard for Safety of Flammability of Plastic Materials for
EN ISO 13849-1:2016-06, Safety of machinery - Safety-related Parts in Devices and Appliances testing
parts of control systems - Part 1: General principles for design
(ISO 13849-1:2015) Other References
EN 61000-6-2:2005-02
DIN EN 61000-6-2:2005-02, Electromagnetic compatibility Bewertungssystem Nachhaltiges Bauen (BNB)
(EMC) - Part 6-2: Generic standards- Immunity for industrial BBSR table (german): 'Nutzungsdauern von Bauteilen zur
environments (IEC 77/295/FDIS:2004); German version prEN Lebenszyklusanalyse nach BNB', Bundesinstitut für Bau-,
61000-6-2:2004 Stadt- und Raumforschung, Referat II Nachhaltiges Bauen;
online available under
DIN EN 61000-6-2 Berichtigung 1:2011-06 https://www.nachhaltigesbauen.de/austausch/nutzungsdauern-
DIN EN 61000-6-2 Berichtigung 1:2011-06, Electromagnetic von-bauteilen/
compatibility (EMC) - Part 6-2: Generic standards -
Immunity for industrial environments (IEC 61000-6-2:2005); Database: MLC CUP 2023.1
German version EN 61000-6-2:2005, Corrigendum to DIN EN Sphera Solutions, 'Managed LCA content', Sphera Solutions,
61000-6-2 (VDE 0839-6-2):2006-03 Chicago, US, 2023.
EN 61000-6-3:2007/A1:2011 Software: LCAFE (gaBi)
EN 61000-6-3:2007/A1:2011, Electromagnetic compatibility Website: sphera.com/life-cycle-assessment-lca-software/
(EMC) - Part 6-3: Generic standards - Emission standard for
7 Environmental Product Declaration - Magnetic Autocontrol GmbH - FlowMotion® mWing
IBU Part A IBU Part B
PCR - Part A: Calculation Rules for the Life Cycle Assessment Electronic and physical Access Control Systems, 01.08.2021,
and Requirements on the Project Report according to EN Institut Bauen und Umwelt e.V., www.bau-umwelt.com, 2023
15804+A2:2019, Institut Bauen und Umwelt e.V., www.bau-
umwelt.com, 2023; version 1.3. 7V21511
Versuchsprotokoll - Strom-und Leistungsmessung mit mWing,
Magnetic Autocontrol GmbH, 08.04.2021
8 Environmental Product Declaration - Magnetic Autocontrol GmbH - FlowMotion® mWing
Publisher
Institut Bauen und Umwelt e.V. +49 (0)30 3087748- 0
Hegelplatz 1 info@ibu-epd.com
10117 Berlin www.ibu-epd.com
Germany
Programme holder
Institut Bauen und Umwelt e.V. +49 (0)30 3087748- 0
Hegelplatz 1 info@ibu-epd.com
10117 Berlin www.ibu-epd.com
Germany
Author of the Life Cycle Assessment
Sphera Solutions GmbH +49 711 341817-0
Hauptstraße 111- 113 info@sphera.com
70771 Leinfelden-Echterdingen www.sphera.com
Germany
Owner of the Declaration
Magnetic Autocontrol GmbH +497622695678
Grienmatt 20 hwolf@ac-magnetic.de
79650 Schopfheim https://www.magnetic-
Germany access.com/de-DE/
9 Environmental Product Declaration - Magnetic Autocontrol GmbH - FlowMotion® mWing
