ENVIRONMENTAL PRODUCT DECLARATION
as per ISO 14025 and EN 15804+A2
Owner of the Declaration Uzin Utz SE
Publisher Institut Bauen und Umwelt e.V. (IBU)
Programme holder Institut Bauen und Umwelt e.V. (IBU)
Declaration number EPD-UZI-20230496-IBC1-EN
Issue date 29.01.2024
Valid to 28.01.2029
Film Tapes
Sifloor AG
www.ibu-epd.com | https://epd-online.com
1. General Information
Sifloor AG Film Tapes
Programme holder Owner of the declaration
IBU – Institut Bauen und Umwelt e.V. Uzin Utz SE
Hegelplatz 1 Dieselstraße 3
10117 Berlin 89079 Ulm
Germany Germany
Declaration number Declared product / declared unit
EPD-UZI-20230496-IBC1-EN 1 m2 of: Film Tape
This declaration is based on the product category rules: Scope:
Dispersion adhesives and primers for floor coverings, 01.08.2021 This Environmental Product Declaration is an average EPD for dry
(PCR checked and approved by the SVR) adhesives covering the products: UZIN Sigan 1, UZIN Sigan 2, UZIN Sigan
3, UZIN Sigan Elements, UZIN Sigan Elements Plus, UZIN Sigan
Elements Tape and UZIN Plurafilm ESD.
Issue date The data provided in this EPD refers to the arithmetic mean of the products
mentioned. All products covered by this EPD are manufactured at the
29.01.2024
Sifloor AG plant in Sursee, Switzerland.
The owner of the declaration shall be liable for the underlying information
and evidence; the IBU shall not be liable with respect to manufacturer
Valid to
information, life cycle assessment data and evidences.
28.01.2029
The EPD was created according to the specifications of EN 15804+A2. In
the following, the standard will be simplified as EN 15804.
Verification
The standard EN 15804 serves as the core PCR
Independent verification of the declaration and data according to ISO
14025:2011
internally X externally
Dipl.-Ing. Hans Peters
(Chairman of Institut Bauen und Umwelt e.V.)
Florian Pronold Matthias Schulz,
(Managing Director Institut Bauen und Umwelt e.V.) (Independent verifier)
1 Environmental Product Declaration - Sifloor AG - Film Tapes
2. Product
Name Value Unit
2.1 Product description/Product definition
Synthetic polymer dispersion (solid content) 20-40 %
This EPD comprises dry adhesives of the product category:
Water 10 - 30 %
Film-Tapes. All products considered here are based on the
switchTec dry adhesive technology. This is a technology for Additives 0 - 15 %
floor bonding and fulfils the function of liquid adhesives as an Liner (protective paper) 20 - 35 %
alternative in flooring technology. Carrier material 5 - 25 %
The following products can be assigned to this EPD:
All products covered by this EPD are very low in volatile organic
• UZIN Sigan 1
compound (VOC) emission. They are all certified as EMICODE
• UZIN Sigan 2
EC1 Plus according to the EMICODE requirements.
• UZIN Sigan 3
Furthermore, UZIN Sigan 1, UZIN Sigan 2 and UZIN Sigan 3
• UZIN Sigan Elements
are awarded with the Blue Angel (DE-UZ 113) due to their low
• UZIN Sigan Elements Plus
emissions. Furthermore UZIN Sigan 1, UZIN Sigan 2 and UZIN
• UZIN Sigan Elements Tape
Sigan 3 contain raw materials following the Bio Mass Balance
• UZIN Plurafilm ESD
Approach. However, this approach was not considered for this
For the use and application of the product the respective
EPD.
national provisions at the place of use apply, in Germany for
example the building codes of the federal states and the
REACH regulation:
corresponding national specifications.
Does this product/article/at least one partial article contains
2.2 Application
substances listed in the candidate list (date: 01.01.2024)
The different film tapes are specially adapted to different
exceeding 0.1 percentage by mass?
substrates and floor coverings and are suitable for full-surface
NO
bonding of floor coverings. Substrates that meet the
requirements of DIN 18365 are suitable for the use of dry
Does this product/article/at least one partial article contains
adhesives after levelling. In addition, special dry adhesives are
other CMR substances in categories 1A or 1B which are not on
also suitable for direct application on existing floor coverings.
the candidate list, exceeding 0.1 percentage by mass?
2.3 Technical Data NO
The various foil tapes are specially adapted to different
Were biocide products added to this construction product or
substrates and floor coverings to comply with their
has it been treated with biocide products (this then concerns a
requirements.
treated product as defined by the (EU) Ordinance on Biocide
Constructional data Products No. 528/2012)?
Name Value Unit NO
Dimensional changes (in transverse direction) Information on hazardous substances (if any) contained in this
acc. to ISO 22633 (Dispersion adhesives for product can be found in the product specific Safety Data sheet.
textile and elastic floor coverings, not applicable max. The latest version is available at our Website:
for polyvinyl chloride floor coverings, rubber floor <0.2% % https://int.uzin.com/
coverings, smooth polyolefin floor coverings,
textile floor coverings)
2.6 Manufacture
Dimensional changes acc. to ISO 22635
The ingredients of the adhesive component are first added
(Dispersion adhesives for textile and elastic floor max.
<0.2% together according to the corresponding formula and mixed
coverings, (not applicable for linoleum or textile %
under continuous stirring. In two steps, the adhesive
floor coverings)
component is then first applied to the carrier material on one
Other constructional data are not relevant for this product. side and dried in the drying line. The process is then repeated
for the other side. In order to prevent the film tape from sticking
Performance data of the product with respect to its when it is rolled up, a protective paper (liner) is applied to one
characteristics in accordance with the relevant technical of the adhesive sides.
provision (no CE-marking).
2.7 Environment and health during manufacturing
2.4 Delivery status Apart from the standard precautions for occupational hygiene
All products covered by this EPD are delivered ready to use. and safety, there are no special protective precautions to be
The content of one packaging unit is sufficient for 20 m2 and observed during production.
consists of the film tape (18,75 m2) and an edge tape (1,25 m2).
2.8 Product processing/Installation
An exception to this is the UZIN Sigan Elements Tape, which is
Dry adhesives are applied by hand on appropriately prepared
delivered individually packaged.
substrates. To do so, first the edge tape is installed along walls
2.5 Base materials/Ancillary materials and doors. Then the tapes are rolled out to an area to be
Dry adhesives in general consist of a carrier material with a installed and rubbed in thoroughly with a textile cork rubbing
self-adhesive layer on both sides. On average, the film tapes board. Following, the tape is cut to size with a hook knife.
covered by this EPD are composed of: Afterwards, the protective paper on the opposite side is peeled
off, revealing a second adhesive side. In the last step, the floor
covering can be applied to the second adhesive side by
applying pressure on it.
2 Environmental Product Declaration - Sifloor AG - Film Tapes
2.9 Packaging 2.13 Extraordinary effects
The film tape is wrapped in an additional layer of protective Fire
paper and packed together with the edge tape in a cardboard There are no normative requirements for fire protection for this
packaging. Emptied cores and cardboard packaging are product group. The fire behaviour of the floor construction is
recyclable. The weight and shape of the packaging are different primarily determined by the type and nature of the installed
for the products considered here. More details can be found floor covering or insulation layers. Therefore, the fire resistance
under Section 2.4. class of the floor covering according to EN 13501 must be
taken into account when assessing the fire behaviour. The fire
2.10 Condition of use classification of the floor covering to be installed will be
The substantial composition during the use phase refers to the maintained when installed on switchTec dry adhesives.
composition during the manufacturing. Compared to liquid Water
adhesives, dry adhesives do not harden through chemical Excessive amounts of water can damage the substrate or the
reactions, but are permanently adhesive and do not dry out. floor covering. When the dry adhesive comes into contact with
water, the adhesive strength is weakened and returns to full
2.11 Environment and health during use
strength after the water has fully evaporated. No substances
The products covered by this EPD have been awarded the are washed out that could be hazardous to water.
emission label EMICODE EC 1 PLUS "very low emission". With
the emission label, the dry adhesives contribute to preserving a Mechanical destruction
healthy indoor climate. Details on the individual criteria of the Not of relevance.
EMICODE can be found under point 7 Requisite Evidence.
All products covered by this EPD meet the highest DGNB 2.14 Re-use phase
Quality Level 4. Furthermore, the products contribute to further UZIN SIGAN 1, UZIN SIGAN 2, UZIN SIGAN 3, UZIN SIGAN
green building rating systems such as LEED and BREEAM. ELEMENTS and UZIN SIGAN ELEMENTS PLUS can be
UZIN Sigan 1, UZIN Sigan 2, UZIN Sigan 3, UZIN Sigan removed from the substrate without any residues. However,
Elements, UZIN Sigan Elements Plus and UZIN Sigan adhesive residues may remain on the floor covering but can be
Elements Tape are also provided with the Ü-mark. easily disposed with it. The Tapes can be disposed as
household waste. The re-use of the tapes covered by this EPD
is not possible.
2.12 Reference service life
The service life of dry adhesives depends on the service life of 2.15 Disposal
the floor covering. In turn, the service life of different floor The EWC waste code in accordance with the European Waste
coverings show a high variability (10-50 years according to the Catalogue / List of Waste Ordinance for cured dispersion waste
table "Service lives of components for life cycle assessment bears the EWC waste code 080410 (adhesive and sealing
according to Assessment System for Sustainable Building compound waste). Material residues can be disposed of as
(BNB)"; BBSR: Bundesinstitut für Bau-, Stadt- und household waste.
Raumforschung; www.nachhaltigesbauen.de/baustoff-
undgebaeudedaten/nutzungsdauern-von-bauteilen.html)) 2.16 Further information
Therefore, the specification of a reference service life according Product and safety data sheet, EMICODE EC 1 PLUS and Blue
to ISO 15686 is not possible. Angel certificate, general building authority approval and further
information at https://int.uzin.com/.
3. LCA: Calculation rules
The representativeness of the average LCA values is rated as
3.1 Declared Unit good. Comparability with regard to temporal, geographical and
This declaration is an average EPD and refers to 1 m2 of the technological factors is ensured by the fact that all the products
film tapes UZIN Sigan 1, UZIN Sigan 2, UZIN Sigan 3, UZIN considered here were manufactured in the same plant using
Sigan Elements, UZIN Sigan Elements Plus and UZIN Sigan the same machinery, while the same reference year was
Elements Tape and UZIN Plurafilm ESD, manufactured by utilised. Differences may arise in the exact composition of the
SIFLOOR AG at the Sursee plant. All values stated in this EPD applied adhesive and its coating thickness, as well as the
represent the arithmetic mean of the individual values of the substrate material used.
products. The products mentioned are manufactured at the Further information regarding the variability of specific impact
same plant, fulfil the same or a comparable function and differ indicators is given in Chapter 6.
only slightly in their formulation; other life cycle phases are the
same, such as production and packaging. The declared unit of 3.2 System boundary
1 m2 was chosen as the operating data is recorded either per Type of EPD: Cradle to gate with options, modules C1–C4, and
linear metre [m] or per square metre [m2] and the sales unit is module D (A1–A3 + C + D and additional modules). The
also given in m2. Using the conversion factor of the average additional modules are A4 and A5. The underlying LCA
addresses all life cycle stages of the average product. The
mass per square metre, the data given can be related to 1 kg.
other life cycle stages are not relevant for the product class and
Declared unit and mass reference no environmental impacts occur in these. The following
Name Value Unit activities are covered by the relevant modules:
Declared Unit 1 m2 • A1: Production of raw and auxiliary materials
Gross density 1 - 1.5 kg/m3 • A2: Transport of raw and auxiliary materials to the plant
• A3: Production in the plant (incl. provision of energy and
Grammage (average over all products
0.277 kg/m2 waste treatment) and the manufacture of the packaging
considered)
• A4: Transport of the packed product to the construction
Layer thickness (average over all products
0.0003 m site
considered)
3 Environmental Product Declaration - Sifloor AG - Film Tapes
• A5: Installation of the product and disposal of the flows were neglected with regard to the cut-off criteria.
packaging and waste produced during installation
(including the protective paper) 3.5 Background data
• C1: Manual removal of the product Factory-specific data was used for the production processes.
• C2: Transport for disposal For all other life cycle phases, data sets from Sphera Managed
• C3: As a worst-case scenario thermal treatment of the LCA Content (Content Version 2023.2) were used. The LCA
product in an incineration plant is modelled as end-of- model was created in the software LCA for Experts (Version 10)
life scenario (former GaBi).
• C4: Not relevant because the product is incinerated
3.6 Data quality
(respective impacts declared in C3)
• D: Credits resulting from thermal utilisation of the The data quality can be classified as good. The plant-specific
product and packaging waste data refer to the year 2022. All remaining data originate from
For the environmental impact, the use of green electricity was the above-mentioned database, the contents of which are
calculated taking into account the residual electricity mix for the regularly reviewed to ensure their currency. Thus, the data used
remaining electricity. The proportion of the on-site electricity for the life cycle assessment are representative. For some input
demand covered by green electricity in the total on-site materials, proxy datasets had to be used. All background
electricity demand is 100 %. datasets used are less than 10 years old. Data sets are
complete and comply with the system boundaries and the cut-
off rules for inputs and outputs. The data quality thus meets the
3.3 Estimates and assumptions requirements of PCR Part A.
No material loss was assumed in module A5 (installation), as
3.7 Period under review
this is strongly dependent on the application procedure. In
order to determine the environmental burdens caused by the The year 2022 is used as the reference year.
compensation of the additional material effort due to the
3.8 Geographic Representativeness
material loss, the following scheme can be used: The material
Land or region, in which the declared product system is
loss expressed as a percentage [%] is multiplied by the
manufactured, used or handled at the end of the product´s
indicator values from modules A1-A4 and C3 and added to
lifespan: Europe
module A5. A subtraction of the indicator values from modules
A1-A4 and C3 is not necessary, as only the additional material
effort to compensate for the material loss is considered. 3.9 Allocation
As end-of-life assumption for the packaging and the product, a
Site-specific operating data was distributed to the different
100 % thermal treatment scenario was chosen, respectively.
products according to the machine utilisation.
Since the products considered in this EPD are delivered in
different packaging, the packaging with the least favourable 3.10 Comparability
ratio of packaging weight to product weight was used for the Basically, a comparison or an evaluation of EPD data is only
calculation. possible if all the data sets to be compared were created
according to EN 15804 and the building context, respectively
the product-specific characteristics of performance, are taken
3.4 Cut-off criteria
into account. The background database is used from Sphera
The common rules according to ISO 14044 were applied as
Managed LCA Content. In this EPD, dry adhesives are
cut-off criteria. These apply to the entire product system as well
considered. These differ from liquid dispersion adhesives in
as to individual process modules and take into account mass,
their specific characteristics of performance and response to
energy and environmental relevance. All inputs were included
(punctual) stresses, so a direct comparison is not possible.
in the LCA that are more than 1 % with regard to the total
impact of an impact category. Overall, no more than 5 % of the
4. LCA: Scenarios and additional technical information
Transport to the building site (A4)
Characteristic product properties of biogenic carbon
The transport was divided into two phases, which best
Biogenic carbon content at the gate:
correspond to the actual situation. In the first stage, the product
is transported to a wholesaler by a large truck. The second
Note: 1 kg of biogenic carbon is equivalent to 44/12 kg of CO .
2 stage represents the transport from the wholesaler to the
construction site, which is mostly done by the craftsman with a
Biogenic carbon in the product is only contained in the
small truck.
protective paper used, which reaches the end of its waste
Name Value Unit
properties in A5 and is therefore fully emitted and booked out in
A5 and not in C3. Transport distance (Stage 1) 450 km
Information on describing the biogenic carbon content at Gross weight (Stage 1) 34 - 40 t
factory gate Payload capacity (Stage 1) 27 t
Name Value Unit Utilisation by mass (Stage 1) 0.61 -
Biogenic carbon content in product (arithmetic 3.10E- kg ------------------------------- ----------- ----------- -----
mean) 02 C Transport distance (Stage 2) 50 km
Biogenic carbon content in accompanying 1.87E- kg Gross weight (Stage 2) 7.5 - 12 t
packaging 02 C Payload capacity (Stage 2) 5 t
Utilisation by mass (Stage 2) 0.61 -
In the following, the technical scenario information is presented,
which enables a better understanding of the declared modules.
4 Environmental Product Declaration - Sifloor AG - Film Tapes
A1-A4 and C3 is not necessary, as only the additional material
Installation into the building (A5)
effort to compensate for the material loss is considered.
Name ValueUnit
The protective paper, attached to the product is disposed of
Auxiliary - kg during the installation phase. Thermal treatment was assumed
Water consumption - m3 as a worst-case scenario.
Other resources - kg
Electricity consumption - kWh End of life (C1-C4)
Other energy carriers - MJ Name ValueUnit
Material loss - kg Collected as mixed construction waste (arithmetic
0.187 kg
Output substances following waste treatment on mean)
0.09 kg
site Reuse - kg
Dust in the air - kg Recycling - kg
VOC in the air - kg Energy recovery 100 %
Landfilling 0 %
No material loss was assumed in module A5 (installation), as
this is strongly dependent on the application procedure. In The difference in mass between the product shipped and the
order to determine the environmental burdens caused by the product installed and thus to be disposed of in C3 differs due to
compensation of the additional material effort due to the the protective paper which is removed during installation. The
material loss, the following scheme can be used: The material waste treatment of the protective paper is declared in module
loss expressed as a percentage [%] is multiplied by the A5.
indicator values from modules A1-A4 and C3 and added to
module A5. A subtraction of the indicator values from modules
5 Environmental Product Declaration - Sifloor AG - Film Tapes
5. LCA: Results
DESCRIPTION OF THE SYSTEM BOUNDARY (X = INCLUDED IN LCA; MND = MODULE OR INDICATOR NOT DECLARED; MNR
= MODULE NOT RELEVANT)
Benefits and
Construction loads beyond
Product stage Use stage End of life stage
process stage the system
boundaries
la ire ta m w a Ry lp p u s tro p s n a rT g n iru tc a fu n a M e h t m o rf tro p s n a rTe tis e h t o t e ta g y lb m e s s A e s U e c n a n e tn ia M ria p e R tn e m e c a lp e R tn e m h s ib ru fe R y g re n e la n o ita re p Oe s u re ta w la n o ita re p Oe s u n o itc u rts n o c -e Dn o itilo m e d tro p s n a rT g n is s e c o rp e ts a W la s o p s iD -e s u e R-y re v o c e R-g n ilc y c e Rla itn e to p
A1 A2 A3 A4 A5 B1 B2 B3 B4 B5 B6 B7 C1 C2 C3 C4 D
X X X X X MND MND MNR MNR MNR MND MND X X X MND X
RESULTS OF THE LCA - ENVIRONMENTAL IMPACT according to EN 15804+A2: 1 m^2 Film Tape
Parameter Unit A1-A3 A4 A5 C1 C2 C3 D
GWP-total kg CO 2 eq 7.21E-01 1.27E-02 1.93E-01 0 4.07E-04 2.37E-01 -1.04E-01
GWP-fossil kg CO 2 eq 8.97E-01 1.26E-02 1.18E-02 0 4.02E-04 1.15E-01 -1.04E-01
GWP-biogenic kg CO 2 eq -1.82E-01 2.93E-05 1.82E-01 0 9.35E-07 1.22E-01 -4.68E-04
GWP-luluc kg CO 2 eq 5.07E-03 1.18E-04 3.62E-06 0 3.78E-06 4.91E-06 -6.7E-06
ODP kg CFC11 eq 1.99E-08 1.12E-15 2.84E-14 0 3.57E-17 4.31E-14 -8E-13
AP mol H+ eq 2.5E-03 4.44E-05 7.75E-05 0 1.4E-06 1.24E-04 -1.28E-04
EP-freshwater kg P eq 5.29E-06 4.66E-08 1.44E-08 0 1.49E-09 2.39E-08 -1.65E-07
EP-marine kg N eq 7.03E-04 2.04E-05 2.97E-05 0 6.47E-07 4.82E-05 -3.77E-05
EP-terrestrial mol N eq 7.01E-03 2.3E-04 3.46E-04 0 7.26E-06 5.49E-04 -4.04E-04
kg NMVOC
POCP 2.1E-03 4E-05 7.78E-05 0 1.27E-06 1.26E-04 -1.05E-04
eq
ADPE kg Sb eq 2.94E-06 8.31E-10 2.55E-10 0 2.65E-11 3.72E-10 -7.33E-09
ADPF MJ 2.09E+01 1.74E-01 7.62E-02 0 5.55E-03 1.15E-01 -1.91E+00
m3 world eq
WDP 1.28E-01 1.47E-04 2.19E-02 0 4.71E-06 2.96E-02 -9.7E-03
deprived
GWP = Global warming potential; ODP = Depletion potential of the stratospheric ozone layer; AP = Acidification potential of land and water; EP =
Eutrophication potential; POCP = Formation potential of tropospheric ozone photochemical oxidants; ADPE = Abiotic depletion potential for non-fossil
resources; ADPF = Abiotic depletion potential for fossil resources; WDP = Water (user) deprivation potential)
RESULTS OF THE LCA - INDICATORS TO DESCRIBE RESOURCE USE according to EN 15804+A2: 1 m^2 Film Tape
Parameter Unit A1-A3 A4 A5 C1 C2 C3 D
PERE MJ 5.11E+00 1.23E-02 1.75E+00 0 3.93E-04 3.13E-02 -5.46E-01
PERM MJ 1.74E+00 0 -1.74E+00 0 0 0 0
PERT MJ 6.85E+00 1.23E-02 1E-02 0 3.93E-04 3.13E-02 -5.46E-01
PENRE MJ 1.5E+01 1.74E-01 3.87E-01 0 5.57E-03 5.72E+00 -1.91E+00
PENRM MJ 5.92E+00 0 -3.1E-01 0 0 -5.61E+00 0
PENRT MJ 2.09E+01 1.74E-01 7.7E-02 0 5.57E-03 1.1E-01 -1.91E+00
SM kg 0 0 0 0 0 0 0
RSF MJ 0 0 0 0 0 0 0
NRSF MJ 0 0 0 0 0 0 0
FW m3 6.81E-03 1.36E-05 5.16E-04 0 4.33E-07 7E-04 -4.43E-04
PERE = Use of renewable primary energy excluding renewable primary energy resources used as raw materials; PERM = Use of renewable primary
energy resources used as raw materials; PERT = Total use of renewable primary energy resources; PENRE = Use of non-renewable primary energy
excluding non-renewable primary energy resources used as raw materials; PENRM = Use of non-renewable primary energy resources used as raw
materials; PENRT = Total use of non-renewable primary energy resources; SM = Use of secondary material; RSF = Use of renewable secondary fuels;
NRSF = Use of non-renewable secondary fuels; FW = Use of net fresh water
RESULTS OF THE LCA – WASTE CATEGORIES AND OUTPUT FLOWS according to EN 15804+A2:
1 m^2 Film Tape
Parameter Unit A1-A3 A4 A5 C1 C2 C3 D
HWD kg 3.24E-05 6.45E-13 2.57E-12 0 2.06E-14 4.03E-12 -1.06E-10
NHWD kg 7.69E-02 2.51E-05 1.78E-02 0 8.02E-07 3.24E-02 -9.36E-04
RWD kg 3.98E-04 2.25E-07 3.44E-06 0 7.2E-09 4.99E-06 -1.45E-04
CRU kg 0 0 0 0 0 0 0
MFR kg 0 0 0 0 0 0 0
MER kg 0 0 0 0 0 0 0
EEE MJ 0 0 2.19E-01 0 0 2.64E-01 0
EET MJ 0 0 4.05E-01 0 0 4.95E-01 0
HWD = Hazardous waste disposed; NHWD = Non-hazardous waste disposed; RWD = Radioactive waste disposed; CRU = Components for re-use;
MFR = Materials for recycling; MER = Materials for energy recovery; EEE = Exported electrical energy; EET = Exported thermal energy
6 Environmental Product Declaration - Sifloor AG - Film Tapes
RESULTS OF THE LCA – additional impact categories according to EN 15804+A2-optional:
1 m^2 Film Tape
Parameter Unit A1-A3 A4 A5 C1 C2 C3 D
Disease
PM ND ND ND ND ND ND ND
incidence
IR kBq U235 eq ND ND ND ND ND ND ND
ETP-fw CTUe ND ND ND ND ND ND ND
HTP-c CTUh ND ND ND ND ND ND ND
HTP-nc CTUh ND ND ND ND ND ND ND
SQP SQP ND ND ND ND ND ND ND
PM = Potential incidence of disease due to PM emissions; IR = Potential Human exposure efficiency relative to U235; ETP-fw = Potential comparative
Toxic Unit for ecosystems; HTP-c = Potential comparative Toxic Unit for humans (cancerogenic); HTP-nc = Potential comparative Toxic Unit for humans
(not cancerogenic); SQP = Potential soil quality index
Disclaimer 1 – for the indicator 'Potential Human exposure efficiency relative to U235'. This impact category deals mainly with the
eventual impact of low-dose ionizing radiation on human health of the nuclear fuel cycle. It does not consider effects due to possible
nuclear accidents, occupational exposure or radioactive waste disposal in underground facilities. Potential ionizing radiation from the
soil, radon and from some construction materials is also not measured by this indicator.
Disclaimer 2 – for the indicators 'abiotic depletion potential for non-fossil resources', 'abiotic depletion potential for fossil resources',
'water (user) deprivation potential, deprivation-weighted water consumption', 'potential comparative toxic unit for ecosystems', 'potential
comparative toxic unit for humans – cancerogenic', 'Potential comparative toxic unit for humans - not cancerogenic', 'potential soil
quality index'. The results of this environmental impact indicator shall be used with care as the uncertainties on these results are high
as there is limited experience with the indicator.
Disclaimer 3: Additional environmental impact indicators (EN 15804, Table 4) are not declared in the EPD. The results of these
environmental impact indicators should be used with caution as the uncertainties in these results are high and there is limited
experience with the indicators (see ILCD classification in EN 15804, Table 5). For this reason, the results based on these indicators are
not reported.
6. LCA: Interpretation
for in Module A5 in the form of biogenic CO emissions.
2
The coefficient of variation is a measure of the relative scatter.
It indicates what percentage of the average the standard
deviation is. It is therefore the percentage ratio of the standard
deviation to the arithmetic mean. It is used to make it easier to
compare the spread of different distributions. The spread of the
impact indicators is generally low. Among the impact
assessment indicators, the results for the indicators Climate
Change, land use and land use change, Ozone Depletion and
Water Use show the highest scatter, which is due to differences
in the product formulations analysed.
Alongside the coefficient of variation, the maximum deviation of
individual products' impact from the average value for specific
impact indicators was also analysed (see table below). These
show that some impact indicators such as Ozone Depletion
react sensitively to individual substances contained, resulting in
The dominance analysis of the impact assessment indicators a high deviation. In general, however, the results are in the
shows a large contribution from the manufacturing phase (A1- same order of magnitude, which indicates a appropriate
A3). A large proportion of the environmental impact stems from grouping.
the raw materials used (A1), with the synthetic polymer
dispersions making the highest contributions (with regard to the
impact indicator Climate Change - total, an average of 59% of
the impact in A1 is attributable to this component).
In addition, the waste treatment of the packaging and the
product (A5, C3) plays a major role for the Climate Change -
total impact assessment indicator. In these modules, thermal
utilisation was modelled as a worst-case scenario. The large
proportion in module A5 in particular can be explained by the
fact that in addition to the waste treatment of the packaging, the
waste treatment of the protective paper is also declared in this
module, which on average accounts for one third of the total
mass of the product. Furthermore, both the packaging and the
protective paper contain biogenic carbon, which is accounted
7 Environmental Product Declaration - Sifloor AG - Film Tapes
renewable energy resources contained in the raw materials and
packaging materials with biogenic content.
The coefficients of variation of the life cycle inventory indicators
generally show a low level of scatter. Among the life cycle
inventory indicators, the results for the indicators Hazardous
waste disposed, Non-hazardous waste disposed (NHWD) and
Radioactive waste disposed (RWD) show the highest scatter,
which is due to differences in the product formulations
considered.
The assumptions used to determine the reported impact
indicator results are presented in Chapter 3.3. Specific data
was used for operational activities in phases A2-A3. Raw
material inputs (A1) were mainly modelled using generic
background data sets. Raw material inputs in particular have a
major influence on all the indicators shown, so care was taken
here to use data sets that are representative in terms of
technological aspects. In order to achieve this, also data sets
In relation to the life cycle inventory indicators Total use of were used whose reference year was up to 10 years in the
renewable primary energy resources (PERT) and Total use of past, which led to an overall medium temporal
non-renewable primary energy resources (PENRT), the largest representativeness. With regard to geographical aspects, the
share of energy consumption in the life cycle occurs in the results presented in this EPD are representative for Europe.
manufacturing phase (A1-A3). Significant contributions to Activities in the downstream life cycle phases (A4-A5; C1-C3)
primary energy demand - non-renewable (PENRT) come from were modelled using scenarios, whereby assumptions were
the energy resources contained in the raw materials. The made regarding transport distance, for example. However,
largest contribution to primary energy demand - renewable these life cycle phases are not dominant for the reported impact
(PERT) is the consumption of renewable energy resources indicators.
needed to generate and provide electricity, as well as the
7. Requisite evidence
Technical data sheet, Safety Data Sheet, license of EMICODE according to ISO 16000-11 in a test chamber. Testing for
EC1 PLUS, certificate of the German Blue Angel and other carcinogenic, mutagenic, reprotoxic (CMR) substances and
product-related information are available for download at TVOC/TSVOC after 3 and 28 days.
https://int.uzin.com 7.1 VOC emissions Furthermore, the emission of volatile organic compounds from
building products in accordance with the award criteria for the
TVOC* limit values EMICODE following the AgBB scheme
eco-label "Low-emission floor covering adhesives and other
for EMICODE EC1 Plus (28 days [µg/m³])
flooring installation materials, DE-UZ 113', were determined.
Name Value Unit
TVOC (C6 - C16) ≤ 60 μg/m3 Date of test report: Test report dated 18 December 2019;
Sum SVOC (C16 - C22) ≤ 40 μg/m3
Result: The product complies with the requirements according
R (dimensionless) ≤ 1 -
to the GEV test method for 'EMICODE EC 1 PLUS – very low
VOC without NIK ≤ 40 μg/m3
emissions' classification and fulfils the requirements according
Carcinogenic Substances ≤ 1 μg/m3 to the award basis for DE-UZ 113.
TVOC* limit values BLUE ANGEL DE-UZ 113 following the AgBB scheme
AgBB scheme (28 days [µg/m³]) The requirements on emission performance according to AgBB
Name Value Unit for the ü-mark are automatically regarded as satisfied for
TVOC (C6 - C16) Specific products availing of EMICODE EC 1 PLUS classification.
≤ 60 μg/m3
concentration
Sum SVOC (C16 - C22) Specific
≤ 50 μg/m3
concentration
R (dimensionless) ≤ 1
VOC without LCI Specific concentration ≤ 40 μg/m3
Carcinogenic Substances Specific ≤ 1 per single
μg/m3
concentration value
Acetic acid ≤ 140 μg/m3
Formaldehyde ≤ 0.05 ppm
Other aldehydes ≤ 0.05 ppm
Test institute: Eurofins Product Testing A/S, 8464 Galten,
Denmark
Measuring process: GEV test method for determining the
emissions of volatile organic compounds from building products
8 Environmental Product Declaration - Sifloor AG - Film Tapes
8. References
Standards: BNB
Assessment System for Sustainable Building; https://www.bnb-
DIN 18356 nachhaltigesbauen.de/en/assessment-system/ [2023]
DIN 18356: German construction contract procedures (VOB) -
Part C: General technical specifications in construction BREEAM
contracts (ATV) - Laying of parquet flooring and wood block BREEAM (Building Research Establishment Environmental
flooring. Assessment Methodology);
https://bregroup.com/products/breeam [2023]
EN 13501-1 Candidate list
DIN EN 13501-1:2019, Fire classification of construction List of substances of very high concern for Authorisation,
products and building elements - Part 1: Classification using published in accordance with Article 59(10) of the REACH
data from reaction to fire tests. Regulation, ECHA, www.echa.europa.eu/candidate-list-table
[2023]
EN 15804
EN 15804:2012+A2:2019+AC:2021, Sustainability of DGNB
construction works — Environmental Product Declarations — DGNB – German Sustainable Building Council; www.dgnb.de
Core rules for the product category of construction products. [2023]
ISO 14025 EMICODE
EN ISO 14025:2011, Environmental labels and declarations — GEV (Gemeinschaft Emissionskontrollierte Verlegewerkstoffe,
Type III environmental declarations — Principles and Klebstoffe und Bauprodukte e.V. Düsseldorf);
procedures. www.emicode.com/en [2023]
ISO 14040 EWC
DIN EN ISO 14040: 2006, Environmental management – Life European Waste Catalog established by Commission decision
cycle assessment – Principles and framework (ISO 2000/532/EC. http://www.environment-agency.gov.uk/ [2023]
14040:2006); German and English versions EN ISO
14040:2006. German AgBB
Committee for Health-related Evaluation of Building Products:
ISO 14044 health-related evaluation of emissions of volatile organic
DIN EN ISO 14044: 2006, Environmental management – Life compounds (VOC and SVOC) from building products;
cycle assessment – Requirements and guidelines (ISO www.umweltbundesamt.de/produkte/bauprodukte/agb b.htm
14044:2006); German and English versions EN ISO [2012]
14044:2006.
IBU 2021
ISO 15686 Institut Bauen und Umwelt e.V.: General Instructions for the
DIN ISO 15686:2017, Buildings and constructed assets -- EPD programme of Institut Bauen und Umwelt e.V., Version
Service life planning. DIN EN 13501. 2.0, Berlin: Institut Bauen und Umwelt e.V., www.ibu-epd.com
[2023]
ISO 16000-11
DIN EN ISO 16000-11:2006-06, Indoor air – Part 11: LCA For Experts Software
Determination of the emission of volatile organic compounds LCA For Experts Software system (Version 10) and Database
from building products and furnishings – Sampling, storage of for Life Cycle Engeneering (Content Version 2023.2). Sphera
samples and preparation of test specimens. Solutions GmbH, Leinfelden-Echterdingen [2023]
ISO 22633 LEED
DIN EN ISO 22632:2019, Adhesives - Test methods for LEED (Leadership in Energy and Environmental Design);
adhesives for floor coverings and wall coverings - https://worldgbc.org/ [2023]
Determination of dimensional changes of a linoleum floor
covering in contact with an adhesive. Ordinance on Biocide Products No. 528/2012
Regulation (EU) No 528/2012 of the European Parliament and
ISO 22635 of the Council of 22 May 2012 concerning the making available
Adhesives - Test method for adhesives for plastic or rubber on the market and use of biocidal products [2012]
floor coverings or wall coverings - Determination of dimensional
changes after accelerated ageing. PCR Part A
Product Category Rules for Building-Related Products and
Further References: Services, Part A: Calculation Rules for the Life Cycle
Assessment and Requirements on the Project report, Version
Blue Angel (DE-UZ 113) 1.3, Institut Bauen und Umwelt e.V. [08/2022]
Bundesministerium für Umwelt, Naturschutz und
Reaktorsicherheit, Umweltbundesamt, DE Deutsches Institut für PCR Part B
Gütesicherung und Kennzeichnung e.V.; Jury Ecolabel; Product Category Rules for Construction Products. Part B:
https://www.blauer-engel.de/en [2023] Dispersion adhesives and primers for floor coverings, Version
3, [06/2023]
9 Environmental Product Declaration - Sifloor AG - Film Tapes
REACH 76/769/EEC of the Council and Guidelines 91/155/EEC,
Directive (EG) No. 1907/2006 of the European Parliament and 93/67/EEC, 93/105/EC and 2000/21/EC of the Commission
of the Council dated 18 December 2006 on the registration, [2006]
evaluation, approval and restriction of chemical substances
(REACH), for establishing a European Agency for chemical Ü-mark
substances, for amending Directive 1999/45/EC and for Ü-mark-Übereinstimmungszeichen; https://www.dibt.de/de
annulment of Directive (EEC) No. 793/93 of the Council, [2023]
Directive (EC) No. 1488/94 of the Commission, Guideline
10 Environmental Product Declaration - Sifloor AG - Film Tapes
Publisher
Institut Bauen und Umwelt e.V. +49 (0)30 3087748- 0
Hegelplatz 1 info@ibu-epd.com
10117 Berlin www.ibu-epd.com
Germany
Programme holder
Institut Bauen und Umwelt e.V. +49 (0)30 3087748- 0
Hegelplatz 1 info@ibu-epd.com
10117 Berlin www.ibu-epd.com
Germany
Author of the Life Cycle Assessment
Uzin Utz SE 0731 4097 0
Dieselstraße 3 nachhaltigkeit@uzin-utz.com
89079 Ulm www.uzin-utz.de
Germany
Owner of the Declaration
Uzin Utz SE 0731 4097 0
Dieselstraße 3 nachhaltigkeit@uzin-utz.com
89079 Ulm www.uzin-utz.de
Germany
11 Environmental Product Declaration - Sifloor AG - Film Tapes
