ENVIRONMENTAL PRODUCT DECLARATION
as per ISO 14025 and EN 15804+A2
Owner of the Declaration voestalpine AG
Publisher Institut Bauen und Umwelt e.V. (IBU)
Programme holder Institut Bauen und Umwelt e.V. (IBU)
Declaration number EPD-VOE-20230103-IBC2-EN
Issue date 09.05.2023
Valid to 08.05.2028
Rolled wire rod
voestalpine Wire Rod Austria GmbH
www.ibu-epd.com | https://epd-online.com
1. General Information
voestalpine Wire Rod Austria GmbH Rolled wire rod
Programme holder Owner of the declaration
IBU – Institut Bauen und Umwelt e.V. voestalpine AG
Hegelplatz 1 voestalpine-Straße 3
10117 Berlin 4020 Linz
Germany Austria
Declaration number Declared product / declared unit
EPD-VOE-20230103-IBC2-EN 1 tonne of untreated rolled wire rod
This declaration is based on the product category rules: Scope:
Structural steels, 01.08.2021 This EPD is based on a declared unit of 1 metric tonne of average
(PCR checked and approved by the SVR) voestalpine untreated rolled wire rod produced at the production site in St.
Peter Freienstein (Austria).
The owner of the declaration shall be liable for the underlying information
Issue date and evidence; the IBU shall not be liable with respect to manufacturer
information, life cycle assessment data and evidences.
09.05.2023
The EPD was created according to the specifications of EN 15804+A2. In
the following, the standard will be simplified as EN 15804.
Valid to
08.05.2028 Verification
The standard EN 15804 serves as the core PCR
Independent verification of the declaration and data according to ISO
14025:2011
internally X externally
Dipl.-Ing. Hans Peters
(Chairman of Institut Bauen und Umwelt e.V.)
Florian Pronold Prof. Dr. Birgit Grahl,
(Managing Director Institut Bauen und Umwelt e.V.) (Independent verifier)
1 Environmental Product Declaration - voestalpine Wire Rod Austria GmbH - Rolled wire rod
2. Product
contains around 500 different steel grades and a total number
2.1 Product description/Product definition of 3500 grades can be produced on customers' demands.
Wire rod made by voestalpine in St. Peter Freienstein is the
base product for lots of applications, that require un- or low Performance data of the product with respect to its
alloyed steel in round shape. Wire rod is hot rolled in characteristics in accordance with the relevant technical
dimensions from 5 to 52 mm. provision (no CE-marking).
A large part of the produced wire rod is delivered to 2.4 Delivery status
voestalpines' own drawing facilities Wire Austria, Wire The produced wire rod has a standard diameter range between
Germany, Wire Italy and Special Wire for further processing. 5 and 52 mm. By applying the EN 10108 standard, tight
Many customers use wire rod directly to manufacture finished- tolerances are guaranteed. Due to our state-of-the-art rolling
or semi-finished products. technologies, even stricter tolerances are achieved.
For the use and application of the product the respective
national provisions at the place of use apply, in Germany for Delivery Condition acc. to EN 10027:
example the building codes of the federal states and the
• +U (as rolled)
corresponding national specifications.
2.5 Base materials/Ancillary materials
2.2 Application
100 % of the pre-material for the wire rod rolling process is
Wire rod from voestalpine Wire Rod Austria GmbH is used for a
made by voestalpine Stahl Donawitz GmbH, which is located
variety of applications.
right next to the wire rod rolling mill. The maximum alloyment
The main amount is used for cold heading products.
content is around 5 %.
Typical examples are fasteners, bolts and rivets, ball studs,
high-strength screws and highly loaded shafts for automotive
The steel is produced by one of the two blast furnaces using
lightweight construction. Further important products made out
the Linz-Donawitz-process (oxygen converter), which was
of wire rod are springs, bearings, chains, as well as welding
developed by voestalpine in 1949.
wire.
The steel works from voestalpine in Donawitz uses
Un- and low-alloyed steel grades categories:
approximately 20 % - 30 % of scrap (internal and external) for
• Cold forging steel its steel production.
• Spring steel
• Chain steel Depending on the steel grade and application the liquid steel is
• Bearing steel poured into one of the two continuous casting lines of
• Soft drawing steel voestalpine Stahl Donawitz and rolled over to a square billet
• Saw wire format of 150 mm x 150 mm.
• Prestressing wire
• Machining steel Each billet has a length up to approximately 18 m, a weight up
• Welding wire to 3 tonnes and is transported to the wire rod mill by train.
• Cold-work steel
Market Segments: This product/article/at least one partial article contains
substances listed in the candidate list (date: 16.1.2020)
• Automotive
exceeding 0.1 percentage by mass: no.
• Construction
• Mechanical Engineering
This product/article/at least one partial article contains other
• Energy
carcinogenic, mutagenic, reprotoxic (CMR) substances in
• White goods
categories 1A or 1B which are not on the candidate list,
• others
exceeding 0.1 percentage by mass: no.
2.3 Technical Data
This EPD applies to all wire rod in the condition 'as rolled' from Biocide products were added to this construction product, or it
voestalpine Wire Rod Austria GmbH, which is why a general has been treated with biocide products (this then concerns a
statement about mechanical properties is not possible. The treated product as defined by the (EU) Ordinance on Biocide
technical data given for the products are generic literature data Products No. 528/2012): no.
for steel as described e.g. in Key to Steel. No product specific
2.6 Manufacture
test rules are applicable to the data given:
The billets from voestalpine Stahl Donawitz GmbH are heated
up in the walking beam furnace to reach the required rolling
Constructional data
temperature.
For dimensions up to 23 mm the loop-laying head and cooling
conveyor line is used. The bar in coil line is used to produce
dimensions from 24 mm to 52 mm.
A total number of 36 rolling stands, deform the wire rod to its
final dimension. Waterboxes along the rolling lines ensure that
the required rolling temperatures are achieved.
2.7 Environment and health during manufacturing
The standard product range of voestalpine Wire Rod Austria
2 Environmental Product Declaration - voestalpine Wire Rod Austria GmbH - Rolled wire rod
voestalpine Wire Rod Austria GmbH in St. Peter Freienstein is There is no change in material composition over the service life
certified according to EMAS III, ISO 9001, ISO 50001, ISO of the product. If used as intended, no effects on the
45001 and ISO 14001. As part of the environmental environment are to be expected.
declarations required by EMAS, voestalpine Wire Rod Austria
GmbH continuously publishes environmentally relevant data 2.11 Environment and health during use
and facts about the site. During the use of wire rod products, no effects on human and
animal health and no harmful emissions to air, soil and water
At the St. Peter Freienstein site, investments are constantly are expected.
being made in the expansion of environmental protection
2.12 Reference service life
measures in order to be able to reduce emissions to air and
water to a minimum. Due to the variety of applications and their stresses,
voestalpine Wire Rod Austria GmbH does not specify a
All operating facilities that have been approved in accordance reference service life for wire rod products. Corrosive
with the environmental impact assessment procedure are also atmospheres must be avoided to guarantee a full lifetime of
periodically inspected by the authorities as part of functionality.
environmental inspections.
2.13 Extraordinary effects
2.8 Product processing/Installation Fire
Wire Rod products from voestalpine Wire Rod Austria GmbH Steel wire rod is not flammable, therefore no flammable gases
are processed by a broad range of different customers in the or vapours escape.
respective factories. Depending on the desired application, the
wire rod is further processed in different ways, e.g. drawing, Water
cold heading, turning, bending or spring coiling. No negative consequences for the environment are to be
expected under the influence of water.
2.9 Packaging
Wire rod is mostly delivered by truck or train. For selected Mechanical destruction
customers voestalpine Wire Rod Austria is also able to supply Unpredictable mechanical impact on the declared products has
by ship. no negative consequences on the environment due to the
plastic deformability of steel.
The products are delivered in coil shape either as a single
2.14 Re-use phase
bundle (3 t coil) or double bundle (2 x 1,5 t coils). These
bundles are strapped together using metal straps to ensure a The declared products from voestalpine Wire Rod Austria
stable position on the trucks/train. GmbH consist of almost 100 % steel and can therefore be
reused or recycled in the steel industry as a secondary raw
In case the coils are loaded on a ship a seaproof packaging is material for an unlimited number of circles.
applied on the wire rod by wrapping it in plastic foil.
2.15 Disposal
The declared product can be fully used as a recycling raw
This EPD considers steel bands as packaging. The majority of
material. The waste code according to the European Waste
products is delivered without additional packaging.
Catalogue is: 17 04 05 (iron and steel). The waste type is
equivalent to the key number 35103 according to the nationally
Coil dimensions:
applicable Waste Catalogue by-law.
• Inner diameter ~ 850 mm
• Outer diameter ~ 1250 mm 2.16 Further information
• Length ~ 2 x 1200 mm or 1 x 2400 mm Further information on the product is available on the website at
• Weight: ~ 2 x 1,5 t or 1 x 3 t https://www.voestalpine.com/wiretechnology/en/contact/production-
ites/voestalpine-wire-rod-austria/
2.10 Condition of use
3. LCA: Calculation rules
mass-specific scaling factor.
3.1 Declared Unit
This environmental product declaration refers to a declared unit 3.2 System boundary
of 1 tonne of average untreated rolled wire rod. The life cycle assessment of average untreated rolled wire rod
refers to a cradle-to-gate analysis with modules (A1–A3 + C
Declared unit
+D). Subsequent life cycle phases are part of the analysis:
Name Value Unit
Declared unit 1 t Module A1–A3 | Production stage
Density 7850 kg/m3 The production stage includes the burdens of the production of
untreated rolled wire rod of voestalpine Wire Rod Austria GmbH
For the calculation of the declared average, input and
at the production site in St. Peter Freienstein. The used steel
production quantities for the entire calendar year 2018 were
billets are provided by the integrated steel mill at the production
taken into account and broken down to the declared product
site in Donawitz. Thus, the upstream environmental impact of
group. The calculated results can thus be considered
the steel supplied is represented by primary data of the
representative for the declared product portfolio of untreated
respective production site. Material and energy flows for the
rolled wire rod of voestalpine Wire Rod Austria GmbH.
rolling line are considered.
Electricity at St. Peter Freienstein is provided from the network
A linear correlation of the environmental impacts with the
of the integrated steel mill at the production site in Donawitz.
product weight is to be expected. Therefore, the conversion
The power plant is represented based on the site-specific
from the declared unit to a specific product is possible using a
conditions. Data for the representation of the power plant refers
3 Environmental Product Declaration - voestalpine Wire Rod Austria GmbH - Rolled wire rod
to the year 2017. Since 2020, Donawitz purchases 100 %
green electricity, which is also considered in this EPD. Thermal 3.5 Background data
energy provision is based on natural gas. Module A1–A3 also This study uses generic background data for the evaluation of
includes the production of the packaging. upstream environmental impacts from GaBi-database 2021.1
and is modelled in GaBi-software version 10.
Module C1 | Deconstruction and demolition
3.6 Data quality
It is assumed that the product is not connected with other
materials and can therefore be dismantled. Associated efforts The foreground data collected at voestalpine Wire Rod Austria
are negligible, no environmental impacts from the GmbH are based on the quantities used and volumes produced
deconstruction of the products are declared. annually. Process data were collected by voestalpine in the
course of reporting to official agencies. Data on material and
Module C2 | Transport energy use originate from material-specific throughput
The transport to the disposal of the material is estimated measurements of various processes as well as from controlling.
declaring a 50 km radius to the waste processing. The technological, geographical and time-related
representativeness of the data base was kept in mind when
Module C3 | Waste processing selecting background data. Whenever specific data were
Product flows that reach Module D for recycling leave the missing, either generic datasets or representative average data
product system in C3. Environmental impacts resulting from the were used instead. The implemented GaBi background
grinding and sorting of steel scrap are not included due to the datasets are not more than ten years old.
negligible expected environmental impact.
3.7 Period under review
Foreground data were collected in the 2018 production year,
Module C4 | Landfilling
and the data are based on the volumes produced on an annual
Module C4 declares the environmental impacts incurred by
basis.
landfilling (5 % of the product).
3.8 Geographic Representativeness
Module D | Benefits and loads beyond the system
Land or region, in which the declared product system is
boundary
manufactured, used or handled at the end of the product´s
The potential for substituting primary steel with a recycling
lifespan: Austria
scenario (95 % of the product) is outlined in Module D.
3.3 Estimates and assumptions
3.9 Allocation
All assumptions are verified through detailed documentation
The primary data for the upstream production of the steel billets
and correspond to the best possible representation of reality
were allocated using the partitioning approach developed by
based on the available data. Regional applicability of the used
worldsteel 2014 for calculating life cycle inventories of co-
background data refers to average data under European or
products in steel production, which is in line with the provisions
German conditions taken from the GaBi-database. German
of EN 15804. The so-called partitioning approach provides for
data were used for the Austrian market whenever European or
the allocation of environmental effects on the steelmaking
Austrian average data were not available.
process and the emerging byproducts based on physical
relations. Material-inherent flow properties are, thus, taken into
3.4 Cut-off criteria
account.
All inputs and outputs for which data are available are included
in the LCA model. Data gaps are filled with conservative
Economic allocation is not considered as referring byproducts
assumptions from average data (when available) or with
and co-products are not directly tradable goods. Furthermore,
generic data and are documented accordingly. Only data with a
long-term contracts for the sale of the byproducts exist, and the
contribution of less than 1 % were cut off. Ignoring such data is
negotiated prices are, therefore, not subject to market
justified based on the irrelevance of the expected effect.
dynamics.
Processes, materials, or emissions known to make a significant
contribution to the environmental effects of the products under 3.10 Comparability
examination have not been neglected. All relevant data were
Basically, a comparison or an evaluation of EPD data is only
collected comprehensively. It is assumed that the data have
possible if all the data sets to be compared were created
been completely recorded and the overall total of ignored input
according to EN 15804 and the building context, respectively
flows do not amount to more than 5 % of total energy and mass
the product-specific characteristics of performance, are taken
flows. Environmental impacts of machines, plant and
into account. The GaBi background database was used to
infrastructure were not included.
calculate the LCA (GaBi 10; 2021.1).
4. LCA: Scenarios and additional technical information
Name Value Unit
Characteristic product properties of biogenic carbon
Packaging (steel coil) 7.84 kg
The declared product does not contain any biogenic carbon.
The considered packaging does not contain any biogenic The end-of-life scenario used in this LCA study is based on the
carbon either. following assumptions and thus complies with the specifications
published in ökobaudat 2022:
End of life (C1–C4)
Name Value Unit
Installation into the building (A5)
Collected separately (steel) 1000 kg
The end-of-life of the packaging materials is not declared in
Recycling 95 % 950 kg
Module A5.
Landfilling 5 % 50 kg
4 Environmental Product Declaration - voestalpine Wire Rod Austria GmbH - Rolled wire rod
This scenario contains a recycling rate of 95 %. Since
Reuse, recovery and/or recycling potentials (D), relevant
voestalpine externally purchases scrap for steel production, this
scenario information
is offset against the steel scrap for recycling (net flow).
Name Value Unit
Net flow of steel scrap 908 kg
5 Environmental Product Declaration - voestalpine Wire Rod Austria GmbH - Rolled wire rod
5. LCA: Results
The following table contains the LCA results for a declared unit of 1 tonne of untreated rolled wire rod.
DESCRIPTION OF THE SYSTEM BOUNDARY (X = INCLUDED IN LCA; ND = MODULE OR INDICATOR NOT DECLARED; MNR =
MODULE NOT RELEVANT)
Benefits and
Construction loads beyond
Product stage Use stage End of life stage
process stage the system
boundaries
la ire ta m w a Ry lp p u s tro p s n a rT g n iru tc a fu n a M e h t m o rf tro p s n a rTe tis e h t o t e ta g y lb m e s s A e s U e c n a n e tn ia M ria p e R tn e m e c a lp e R tn e m h s ib ru fe R y g re n e la n o ita re p Oe s u re ta w la n o ita re p Oe s u n o itc u rts n o c -e Dn o itilo m e d tro p s n a rT g n is s e c o rp e ts a W la s o p s iD -e s u e R-y re v o c e R-g n ilc y c e Rla itn e to p
A1 A2 A3 A4 A5 B1 B2 B3 B4 B5 B6 B7 C1 C2 C3 C4 D
X X X MND MND MND MND MNR MNR MNR MND MND X X X X X
RESULTS OF THE LCA - ENVIRONMENTAL IMPACT according to EN 15804+A2: 1 tonne untreated rolled wire rod
Parameter Unit A1-A3 C1 C2 C3 C4 D
Global Warming Potential total (GWP-total) kg CO 2 eq 2.75E+03 0 3.02E+00 0 2.42E+00 -1.54E+03
Global Warming Potential fossil fuels (GWP-fossil) kg CO 2 eq 2.74E+03 0 3E+00 0 2.44E+00 -1.54E+03
Global Warming Potential biogenic (GWP-biogenic) kg CO 2 eq 8.1E+00 0 -3.56E-03 0 -2.5E-02 -9.97E-01
Global Warming Potential luluc (GWP-luluc) kg CO 2 eq 8.75E-01 0 2.44E-02 0 2.44E-03 2.23E-01
Depletion potential of the stratospheric ozone layer (ODP) kg CFC11 eq 7.06E-12 0 5.9E-16 0 5.77E-15 -2.57E-12
Acidification potential of land and water (AP) mol H+ eq 8.76E+00 0 9.92E-03 0 7.78E-03 -2.76E+00
Eutrophication potential aquatic freshwater (EP-freshwater) kg P eq 9.78E-03 0 8.88E-06 0 1.86E-06 -3.15E-04
Eutrophication potential aquatic marine (EP-marine) kg N eq 2.13E+00 0 4.55E-03 0 1.93E-03 -4.12E-01
Eutrophication potential terrestrial (EP-terrestrial) mol N eq 2.29E+01 0 5.08E-02 0 2.12E-02 -4.01E+00
Formation potential of tropospheric ozone photochemical oxidants kg NMVOC
7.25E+00 0 8.94E-03 0 6.08E-03 -2.11E+00
(POCP) eq
Abiotic depletion potential for non fossil resources (ADPE) kg Sb eq 5E-03 0 2.65E-07 0 1.68E-07 -3.35E-03
Abiotic depletion potential for fossil resources (ADPF) MJ 2.34E+04 0 3.98E+01 0 3.56E+01 -1.34E+04
m3 world eq
Water use (WDP) 2.51E+02 0 2.77E-02 0 -2.89E-02 -3.02E+02
deprived
RESULTS OF THE LCA - INDICATORS TO DESCRIBE RESOURCE USE according to EN 15804+A2: 1 tonne untreated rolled
wire rod
Parameter Unit A1-A3 C1 C2 C3 C4 D
Renewable primary energy as energy carrier (PERE) MJ 1.44E+03 0 2.29E+00 0 2.57E+00 1.23E+03
Renewable primary energy resources as material utilization
MJ 0 0 0 0 0 0
(PERM)
Total use of renewable primary energy resources (PERT) MJ 1.44E+03 0 2.29E+00 0 2.57E+00 1.23E+03
Non renewable primary energy as energy carrier (PENRE) MJ 2.35E+04 0 4E+01 0 3.56E+01 -1.34E+04
Non renewable primary energy as material utilization (PENRM) MJ 0 0 0 0 0 0
Total use of non renewable primary energy resources (PENRT) MJ 2.35E+04 0 4E+01 0 3.56E+01 -1.34E+04
Use of secondary material (SM) kg 9.17E+01 0 0 0 0 9.08E+02
Use of renewable secondary fuels (RSF) MJ 0 0 0 0 0 0
Use of non renewable secondary fuels (NRSF) MJ 0 0 0 0 0 0
Use of net fresh water (FW) m3 1.33E+01 0 2.62E-03 0 3.67E-04 -6.78E+00
RESULTS OF THE LCA – WASTE CATEGORIES AND OUTPUT FLOWS according to EN 15804+A2:
1 tonne untreated rolled wire rod
Parameter Unit A1-A3 C1 C2 C3 C4 D
Hazardous waste disposed (HWD) kg 4.54E-06 0 2.11E-09 0 6.3E-09 3.74E-06
Non hazardous waste disposed (NHWD) kg 2.77E+01 0 6.27E-03 0 5.01E+01 1.61E+02
Radioactive waste disposed (RWD) kg 1.29E-01 0 7.25E-05 0 4.05E-04 4.85E-04
Components for re-use (CRU) kg 0 0 0 0 0 0
Materials for recycling (MFR) kg 0 0 0 9.5E+02 0 0
Materials for energy recovery (MER) kg 0 0 0 0 0 0
Exported electrical energy (EEE) MJ 0 0 0 0 0 0
Exported thermal energy (EET) MJ 0 0 0 0 0 0
RESULTS OF THE LCA – additional impact categories according to EN 15804+A2-optional:
1 tonne untreated rolled wire rod
Parameter Unit A1-A3 C1 C2 C3 C4 D
Disease
Incidence of disease due to PM emissions (PM) ND ND ND ND ND ND
incidence
Human exposure efficiency relative to U235 (IR) kBq U235 eq ND ND ND ND ND ND
Comparative toxic unit for ecosystems (ETP-fw) CTUe ND ND ND ND ND ND
6 Environmental Product Declaration - voestalpine Wire Rod Austria GmbH - Rolled wire rod
Comparative toxic unit for humans (carcinogenic) (HTP-c) CTUh ND ND ND ND ND ND
Comparative toxic unit for humans (noncarcinogenic) (HTP-nc) CTUh ND ND ND ND ND ND
Soil quality index (SQP) SQP ND ND ND ND ND ND
The additional and optional impact categories according to EN 15804+A2 are not declared, as the uncertainty of these indicators is to
be classified as high.
Disclaimer 1 – for the indicator potential human exposure efficiency relative to U235:
This impact category deals mainly with the eventual impact of low dose ionizing radiation on human health of the nuclear fuel cycle. It
does not consider effects due to possible nuclear accidents, occupational exposure nor radioactive waste disposal in underground
facilities. Potential ionizing radiation from the soil, from radon and from some construction materials is also not measured by this
indicator.
Disclaimer 2 – for the indicators abiotic depletion potential for non-fossil resources, abiotic depletion potential for fossil resources, water
(user) deprivation potential, deprivation weighted water consumption, eutrophication fraction of nutrients reaching freshwater end
compartment, potential comparative toxic unit for humans cancerogenic, potential comparative toxic unit for humans not cancerogenic,
potential soil quality index: The results of this environmental impact indicator shall be used with care as the uncertainties on these
results are high or as there is limited experience with the indicator.
6. LCA: Interpretation
The following interpretation contains a summary of the LCA rolled wire rod.
results referenced to a declared unit of 1 tonne of untreated
A comparison of the individual lifecycle phases results in a clear Most of the potential environmental impacts of the production
dominance of the production phase (modules A1–A3). The phase (module A1–A3) of the untreated rolled wire rod can be
environmental effects in the production phase are mainly traced back to the billet production in Donawitz. The production
dominated by the direct process emissions of billet production. of untreated rolled wire rod at the production site at St. Peter
As a result of product recyclability, the material removed at the Freienstein contributes app. 5 % to global warming potential.
end of life can substitute primary steel. According to the set
method, the first step is to saturate the secondary material used A linear correlation of the environmental impacts with the
in module A withmaterial from module C. The excess amount product weight is to be expected. Therefore, the conversion
from module C ('net flow') can substitute primary steel and from the declared unit to a specific product is possible using a
leads to corresponding substitution potentials in module D. mass-specific scaling factor.
The environmental impact of the transport of the products to
recycling (C2) as well as landfilling of the losses at the end of All primary data were specifically broken down to the declared
life (C4) represents a minor contribution to the overall product group. As a result, the representativity of the results for
environmental impact of the product. the declared product group is to be expected as high.
7. Requisite evidence
7 Environmental Product Declaration - voestalpine Wire Rod Austria GmbH - Rolled wire rod
Not relevant for this EPD.
8. References
Standards 761/2001 and Commission Decisions 2001/681/EC and
2006/193/EC.
EN 10027-1
DIN EN 10027-1:2016, Designation systems for steels - Part 1: European Waste Catalogue
Steel names. Guidance on classification of waste according to EWC Stat
categories. Supplement to the Manual for the Implementation of
EN 10108 the Regulation (EC) No 2150/2002 on Waste Statistics.
DIN EN 10108:2004, Round steel rod for cold heading and cold Commission of the European Communities, EUROSTAT.
extrusion Dimensions and tolerances.
GaBi
EN 15804 GaBi 10, Software System and Database for Life Cycle
DIN EN 15804:2012+A2:2019+AC:2021, Sustainability of Engineering. DB 2021.1. Sphera, 1992-2021. Available in:
construction works - Environmental product declarations - Core http://documentation.gabisoftware.com
rules for the product category of construction products.
IBU 2021
ISO 9001 Institut Bauen und Umwelt e.V.: General guidance for the EPD
DIN EN ISO 9001:2015-11, Quality management systems - program of the Institut Bauen und Umwelt e.V.. (IBU). Version
Requirements. 2.0, Berlin: Institut Bauen und Umwelt e.V., 2021.
www.ibu-epd.com
ISO 14001
DIN EN ISO 14001:2015-11, Environmental management Key to Steel
systems - requirements with guidance for use. Key to Steel (Stahlschlüssel) 2019, 25. edition, 2023, Verlag
Stahlschlüssel Wegst GmbH, Germany.
ISO 14025
DIN EN ISO 14025:2011-10, Environmental labels and ökobaudat 2022
declarations - Type III environmental declarations - Principles ökobaudat 2022. EN 15804 and BNB compliant data for over
and procedures. 700 building products.
ISO 14044 Ordinance on Biocide Products
DIN EN ISO 14044:2006-10, Environmental management - Life Regulation (EU) No 528/2012 of the European Parliament and
cycle assessment - Requirements and guidance. of the Council of 22 May 2012 concerning the making available
on the market and use of biocidal products.
ISO 45001
DIN EN ISO 45001:2018-03, Occupational health and safety PCR Part A
management systems - Requirements with guidance for use. Product category rules for building-related products and
services. Part A: Calculation rules for life cycle assessment and
ISO 50001 project report requirements according to EN 15804+A2:2019.
DIN EN ISO 50001:2018-12, Energy management systems - Version 1.3. Berlin: Institut Bauen und Umwelt e.V.. (ed.), 2022.
Requirements with guidance for use.
PCR: Structural steels
Further references Product category rules for building-related products and
services. Part B: Requirements for the EPD for structural steels.
Candidate list Version v0. Berlin: Institut Bauen und Umwelt e.V., 08.03.2023.
Candidate List of Substances of Very High Concern (ECHA
Candidate List) of 16.01.2020, published in accordance with worldsteel 2014
Article 59 (10) of the REACH Regulation Helsinki: European World Steel Association, February 14, 2014: A methodology to
Chemicals Agency. determine the LCI
of steel industry co-products.
EMAS III
Regulation (EC) No 1221/2009 of the European parliament and worldsteel 2019
of the council of 25 November 2009 on the voluntary World Steel Association, 2019: Life cycle inventory
participation by organisations in a Community eco-management methodology report.
and audit scheme (EMAS), repealing Regulation (EC) No
8 Environmental Product Declaration - voestalpine Wire Rod Austria GmbH - Rolled wire rod
Publisher
Institut Bauen und Umwelt e.V. +49 (0)30 3087748- 0
Hegelplatz 1 info@ibu-epd.com
10117 Berlin www.ibu-epd.com
Germany
Programme holder
Institut Bauen und Umwelt e.V. +49 (0)30 3087748- 0
Hegelplatz 1 info@ibu-epd.com
10117 Berlin www.ibu-epd.com
Germany
Author of the Life Cycle Assessment
Daxner & Merl GmbH +43 676 849477826
Schleifmühlgasse 13/24 office@daxner-merl.com
1040 Wien www.daxner-merl.com
Austria
Owner of the Declaration
voestalpine AG +43/50304/15-0
voestalpine-Straße 3 info@voestalpine.com
4020 Linz www.voestalpine.com
Austria
9 Environmental Product Declaration - voestalpine Wire Rod Austria GmbH - Rolled wire rod
