ENVIRONMENTAL PRODUCT DECLARATION
as per ISO 14025 and EN 15804+A2
Owner of the Declaration Fletco Carpets A/S
Publisher Institut Bauen und Umwelt e.V. (IBU)
Programme holder Institut Bauen und Umwelt e.V. (IBU)
Declaration number EPD-FLE-20240140-CBA1-DE
Issue date 29.11.2024
Valid to 28.11.2029
Woven carpet tiles, pile material polyamide 6.6 maximum total pile
weight 510 g/m²
Fletco Carpets A/S
www.ibu-epd.com | https://epd-online.com
General Information
Fletco Carpets A/S Woven carpet tiles, pile material polyamide 6.6
maximum total pile weight 510 g/m²
Programme holder Owner of the declaration
IBU – Institut Bauen und Umwelt e.V. Fletco Carpets A/S
Hegelplatz 1 Mads Clausens Vej 2
10117 Berlin 7441 Bording
Germany Denmark
Declaration number Declared product / declared unit
EPD-FLE-20240140-CBA1-DE 1 m2 woven TEXtile carpet having a pile material of Polyamide 6.6
This declaration is based on the product category rules: Scope:
Floor coverings, 01.08.2021 The manufacturer declaration applies to a group of products with a
(PCR checked and approved by the SVR) maximum total pile weight of 510 g/m2. The carpet is woven at the fletco
manufacturing site in Bording, Denmark. Dyeing and backing of the carpet
is carried out externally
Issue date The declaration is only valid in conjunction with a valid GUT-PRODIS
license of the specific product.
29.11.2024
LCA results for products of the same construction but with a maximum total
Valid to pile weight of 400 g/m2 can be taken from the corresponding tables of the
annexe. Specific data for every product within the declared group of
28.11.2029 products in relation to its total pile weight can be calculated by using
equation 1 given in the annexe (see annexe chapter: 'General Information
on the annexe').
The owner of the declaration shall be liable for the underlying information
and evidence; the IBU shall not be liable with respect to manufacturer
information, life cycle assessment data and evidences.
The EPD was created according to the specifications of EN 15804+A2. In
the following, the standard will be simplified as EN 15804.
Verification
Dipl.-Ing. Hans Peters
The standard EN 15804 serves as the core PCR
(Chairman of Institut Bauen und Umwelt e.V.)
Independent verification of the declaration and data according to ISO
14025:2011
internally X externally
Florian Pronold Angela Schindler,
(Managing Director Institut Bauen und Umwelt e.V.) (Independent verifier)
1 Environmental Product Declaration - Fletco Carpets A/S - Woven carpet tiles, pile material polyamide 6.6 maximum total pile weight 510 g/m²
Product
Performance data of the product in accordance with the
Product description/Product definition declaration of performance with respect to its essential
Flat woven carpet tiles having a pile material of polyamide 6.6 characteristics according to EN 14041: 2018-05, Resilient,
(PA 6.6) and a TEXtile backing. The declaration applies to a textile and laminate floor coverings - Essential characteristics.
group of products with amaximum total pile weight of 510 g/m2. Additional product properties in accordance with EN 1307 can
The recycled content out of total weight amounts to a minimum be found on the Product Information System PRODIS using the
16 %. The surface of the carpet is dyed using aqueous dyeing PRODIS registration number of the product (www.pro-dis.info)
methods. or on the manufacturer's technical information section.
LCA results for products with a maximum total pile weight of Base materials/Ancillary materials
400 g/m2 can be taken from the corresponding tables of the Name Value Unit
annexe. Results for specific products with any other total pile Polyamide 6.6 15,9 %
weight can be calculated by using equation 1 given in the
Polymer dispersion (solid content) 6,5 %
annexe (see annexe chapter: 'General Information on the
Polyester (PET) 24,4 %
annexe').
For the placing on the market of the specific product in the Mineral filler 28,1 %
European Union/European Free Trade Association (EU/EFTA) Aluminium hydroxide 4,6 %
(with the exception of Switzerland) Regulation (EU) No. Low-density polyethylene 18,7 %
305/2011 Construction Product Regulation (CPR) applies. The
Glass fibre 1,1 %
product needs a Declaration of Performance (DoP) taking into
Additives 0.9 %
consideration EN 14041:2018-05, Resilient, textile and laminate
floor coverings - Essential characteristics, and the CE-marking. The specific product covered by the EPD contains substances
The DoP of the product can be found on the manufacturer's listed in the ECHA candidate list (23.01.2024) or other
technical information section. For the application and use of the carcinogenic, mutagenic or reprotoxic (CMR) substances in
product the respective national provisions apply. categories 1A or 1B which are not on the candidate list
exceeding 0.1 percentage by mass: no
Application The products are registered in the GUT-PRODIS Information
According to the use class as defined in EN 1307 the products System. The PRODIS system ensures compliance with
can be used in all professional areas with heavy use which limitations of various chemicals and Volatile Organic Compound
require class 33 or less. (VOC)-emissions and a ban on the use of all substances that
are listed as 'Substances of Very High Concern' (SVHC) under
REACH.
Reference service life
The service life of textile floor coverings strongly depends on
Technical Data
the correct installation taking into account the declared use
classification and the adherence to cleaning and maintenance
Constructional data according to EN 1307 instructions.
A calculation of the reference service life according to ISO
Name Value Unit
15686 is not possible. Alternatively, a reference service life of
Product Form Tiles 50 cm x 50 cm -
10 years can be assumed, during which the functional and
Type of
Woven carpet - visual quality is guaranteed (BNB, Nutzungsdauer von
manufacture
Bauteilen). The technical service life can be significantly longer.
Dyeing method Continuous dyeing -
Yarn type Polyamide 6.6 -
TEXtiles (heavy tile backing with a
Secondary backing -
recycled PET felt)
Total pile weight
510 g/m²
max.
Total carpet weight
3220 g/m2
max.
LCA: Calculation rules
floor covering.
Declared Unit
Other declared units are allowed if the conversion is shown
Name Value Unit transparently.
Declared unit 1 m2
Grammage 3.22 kg/m2
Layer thickness 0.0045 m System boundary
Gross density 715 kg/m3 Type of EPD:
Cradle-to-gate with options, modules C1-C4, module D, and
The declared unit refers to 1 m2 produced textile floor covering. additional modules A4, A5, B1, B2.
The Output of module A5 'Assembly' is 1 m2 installed textile
2 Environmental Product Declaration - Fletco Carpets A/S - Woven carpet tiles, pile material polyamide 6.6 maximum total pile weight 510 g/m²
System boundaries of modules A, B, C, D: declared.
Modules C3, C4 and D are indicated separately for three end-
of-life scenarios: C1 De-construction:
0 - landfill disposal The floor covering is de-constructed manually and no additional
1 - municipal waste incineration environmental impact is caused.
2 - recovery in a cement plant
C2 Transport:
A1-A3 Production: Transport of the carpet waste to a landfill, to the municipal
Energy supply and production of the basic material, processing waste incineration plant (MWI) or to the waste collection facility
of secondary material, auxiliary material, transport of the for recycling.
material to the manufacturing site, emissions, waste water
treatment, packaging material and waste processing up to the C3 Waste processing:
landfill disposal of residual waste (except radioactive waste). C3: Landfill disposal needs no waste processing.
Benefits for generated electricity and steam due to the C3-1: Impact from waste incineration (plant with R1>0.6),
incineration of production waste are aggregated. generated electricity and steam are listed in the result table as
exported energy.
A4 Transport: C3-2: Collection of the carpet waste for recovery in the cement
Transport of the packed textile floor covering from factory gate industry, waste processing (granulating), transport to the
to the place of installation. cement plant, emissions from the incineration.
A5 Installation: C4 Disposal:
Installation of the textile floor covering, processing of C4: Impact from landfill disposal,
installation waste and packaging waste up to the landfill C4-1: The carpet waste leaves the system in module C3-2,
disposal of residual waste (except radioactive waste), the C4-2: The pre-processed carpet waste leaves the system in
production of the amount of carpet that occurs as installation module C3-3.
waste including its transport to the place of installation.
Generated electricity and steam due to the incineration of D Recycling potential:
waste are listed in the result table as exported energy. Calculated benefits result from materials exclusive secondary
Preparation of the floor and auxiliary materials (adhesives, materials (net materials).
fixing agents, PET connectors) are beyond the system D: Benefits for generated energy due to landfill disposal of
boundaries and not taken into account. carpet waste at the end of life,
D-1: Benefits for generated energy due to incineration of carpet
B1 Use: waste at the end-of-life (incineration plant with R1 > 0.6),
Indoor emissions during the use stage. After the first year, no D-2: Benefits for saved fossil energy and saved inorganic
product-related Volatile Organic Compound (VOC) emissions material due to recovery of the carpet in a cement plant.
are relevant due to known VOC decay curves of the product. D-3: Benefits for generated energy due to incineration of
packaging and
B2 Maintenance: installation waste (incineration plant with R1 > 0.6),
Cleaning of the textile floor covering for a period of 1 year:
Vacuum cleaning – electricity supply Geographic Representativeness
Wet cleaning – electricity, water consumption, production of the Land or region, in which the declared product system is
cleaning agent, waste water treatment. manufactured, used or handled at the end of the product´s
The declared values in this module have to be multiplied by the lifespan: Europe
assumed service life of the floor covering in the building in
question.
Comparability
Basically, a comparison or an evaluation of EPD data is only
B3 - B5:
possible if all the data sets to be compared were created
The modules are not relevant within the assumed reference
according to EN 15804 and the building context, respectively
service life of 10 years.
the product-specific characteristics of performance, are taken
into account. Background data are taken from the Sphera MLC
B6 - B7:
database 2023-2. Remaining data gaps are covered by the
No energy and water input are required for the operation of the
ecoinvent 3.9
carpet in the use stage. The modules are not relevant and not
LCA: Scenarios and additional technical information
Transport to the construction site (A4)
Characteristic product properties of biogenic carbon
Name Value Unit
Name ValueUnit Litres of fuel (truck, EURO 0-6 mix) 0.0089 l/100km
kg Transport distance 700 km
Biogenic carbon content in product at factory gate -
C Capacity utilisation (including empty runs) 55 %
Biogenic carbon content in accompanying kg Gross density of products transported 715 kg/m3
0.04
packaging at factory gate C
Installation in the building (A5)
1 kg of biogenic carbon is equivalent to 44/12 kg of CO .
2
Name Value Unit
Material loss 0.097 kg
3 Environmental Product Declaration - Fletco Carpets A/S - Woven carpet tiles, pile material polyamide 6.6 maximum total pile weight 510 g/m²
Cardboard packaging waste is considered to be recycled.
End of Life (C1-C4)
Preparation of the floor and auxiliaries (adhesives, fixing
Three different end-of-life scenarios are declared and the
agents, PET connectors etc.) are not taken into account.
results are indicated separately in module C.
Each scenario is calculated as a 100 % scenario.
Maintenance (B2) Scenario 0: 100 % landfill disposal
The values for cleaning refer to 1 m2 floor covering per year. Scenario 1: 100 % municipal waste incineration (MWI)
Depending on the application based on ISO 10874, the with R1>0.6
technical service life recommended by the manufacturer and Scenario 2: 100 % recovery in the cement industry
the anticipated strain on the floor by customers, the case-
specific useful life can be established. Based on this useful life If combinations of these scenarios have to be calculated this
the effects of module B2 need to be calculated in order to should be done according to the following scheme:
obtain the overall environmental impacts. EOL-impact = x % impact (Scenario 0)
+ y % impact (Scenario 1)
Name Value Unit
+ z % impact (Scenario 2)
Maintenance cycle (vacuum cleaning) 208 Number /year
with x % + y % + z % = 100 %
Maintenance cycle (wet cleaning) 1,5 Number /year
Name ValueUnit
Water consumption (wet cleaning) 0.004 m3
Collected as mixed construction waste (scenarios 0
Cleaning agent (wet cleaning) 0.09 kg and 1) 3,22 kg
Electricity consumption 0.314 kWh Collected separately waste type (scenario 2) 3,22 kg
For further information on cleaning and maintenance see Landfilling (scenario 0) 3,22 kg
www.fletcocarpets.com Energy recovery (scenario 1) 3,22 kg
Energy recovery (scenario 2) 2,134 kg
Recycling (scenario 2) 1,085 kg
Service life
Name Value Unit
Reuse, recovery and/or recycling potentials (D), relevant
Life Span (according to BBSR) 10 a scenario information
Corresponds to the Recovery or recycling potentials due to the three end-of-life
Declared product properties (at
specifications of EN - scenarios (module C) are indicated separately.
the gate) and finishes
1307
An assumed quality of work, Recycling in the cement industry (scenario 2)
Conforms to the
when installed in accordance The organic material of the carpet is used as an alternative fuel
manufacturer's -
with the manufacturer’s in a cement kiln. It mainly substitutes for lignite (68.8 %), hard
instructions
instructions coal (23.6 %) and petrol coke (7.6 %). The inorganic material is
substantially integrated into the cement clinker and substitutes
Usage conditions, e.g. Use in areas defined by
for original material input. VDZ e.V.
frequency of use, mechanical the use class according -
exposure to EN 1307
Maintenance e.g. required According to the
Column D/3 represents module D/A5.
frequency, type and quality and manufacturer's -
replacement of components instructions
4 Environmental Product Declaration - Fletco Carpets A/S - Woven carpet tiles, pile material polyamide 6.6 maximum total pile weight 510 g/m²
LCA: Results
The declared result figures in module B2 have to be multiplied by the assumed service life (in years) of the floor covering in the building
under consideration.
Information on un-declared modules: Modules B3 - B7 are not relevant during the service life of the carpet and are therefore not
declared. Modules C1, C3, C4/1 and C4/2 cause no additional impact (see "LCA: Calculation rules") and are therefore not declared.
Module C2 represents the transport for scenarios 0, 1 and 2. Column D/3 represents module D/A5.
Version number of the characterisation factors used : EN 15804+A2 (based on EF 3.1)
DESCRIPTION OF THE SYSTEM BOUNDARY (X = INCLUDED IN LCA; MND = MODULE OR INDICATOR NOT DECLARED; MNR
= MODULE NOT RELEVANT)
Benefits and
Construction loads beyond
Product stage Use stage End of life stage
process stage the system
boundaries
la ire ta m w a Ry lp p u s tro p s n a rT g n iru tc a fu n a M e h t m o rf tro p s n a rTe tis e h t o t e ta g y lb m e s s A e s U e c n a n e tn ia M ria p e R tn e m e c a lp e R tn e m h s ib ru fe R y g re n e la n o ita re p Oe s u re ta w la n o ita re p Oe s u n o itc u rts n o c -e Dn o itilo m e d tro p s n a rT g n is s e c o rp e ts a W la s o p s iD -e s u e R-y re v o c e R-g n ilc y c e Rla itn e to p
A1 A2 A3 A4 A5 B1 B2 B3 B4 B5 B6 B7 C1 C2 C3 C4 D
X X X X X X X MNR MNR MNR MND MND X X X X X
RESULTS OF THE LCA - ENVIRONMENTAL IMPACT according to EN 15804+A2: 1 m² floor covering
Parameter Unit A1-A3 A4 A5 B1 B2 C1 C2 C3 C3/1 C3/2 C4 C4/1 C4/2 D D/1 D/2 D/3
GWP-total kg CO 2 1.11E 2.43E- 5.15E- 0 5.15E- 0 1.35E- 0 5.76E 5.81E 2.23E- 0 0 0 -1.59E -3.43E- -4.78E-
eq +01 01 01 01 02 +00 +00 01 +00 01 02
GWP-fossil kg CO 2 1.11E 2.4E-01 5.14E- 0 3.15E- 0 1.33E- 0 5.76E 5.8E 2.23E- 0 0 0 -1.59E -3.43E- -4.76E-
eq +01 01 01 02 +00 +00 01 +00 01 02
GWP- kg CO 2 -8.11E- 5.62E- 2.9E-05 0 3.69E- 0 3.12E- 0 3.59E- 5.65E- 0 0 0 0 -7.24E- -1.09E- -2.17E-
biogenic eq 02 04 03 05 04 04 03 04 04
GWP-luluc kg CO 2 4.86E- 2.27E- 2.23E- 0 1.96E- 0 1.26E- 0 1.17E- 4.34E- 1.86E- 0 0 0 -1.03E- -2.05E- -3.1E-06
eq 03 03 04 01 04 04 04 04 04 04
kg
9.11E- 2.15E- 2.73E- 3.42E- 1.19E- 4.08E- 6.83E- -1.25E- -7.04E- -3.74E-
ODP CFC11 0 0 0 3.8E-13 0 0 0
10 14 11 08 15 13 13 11 13 13
eq
mol H+ 1.94E- 1.51E- 7.24E- 7.94E- 8.38E- 3.07E- 3.31E- 6.79E- -1.98E- -1.22E- -5.95E-
AP 0 0 0 0 0 0
eq 02 03 04 04 05 03 03 04 03 03 05
EP- 3.12E- 8.95E- 9.77E- 5.23E- 4.97E- 4.48E- 6.27E- 4.35E- -2.57E- -4.41E- -7.71E-
kg P eq 0 0 0 0 0 0
freshwater 05 07 07 06 08 07 07 05 06 07 08
6.49E- 2.62E- 1.92E- 4.11E- 1.44E- 1.55E- 1.55E- -3.94E- -1.74E-
EP-marine kg N eq 7.4E-04 0 0 0 0 0 0 -5.8E-04
03 04 04 05 03 03 04 04 05
8.21E- 2.84E- 2.77E- 4.56E- 1.67E- 1.79E- 1.71E- -6.21E- -4.32E- -1.86E-
EP-terrestrial mol N eq 6.9E-02 0 0 0 0 0 0
03 03 03 04 02 02 03 03 03 04
kg
8.17E- 4.18E- 9.67E- 7.77E- 3.71E- 3.93E- 4.94E- -1.62E- -4.85E-
POCP NMVOC 2.2E-02 1.4E-03 0 0 0 0 0 -1.2E-03
04 04 04 05 03 03 04 03 05
eq
1.14E- 1.59E- 3.51E- 2.14E- 8.85E- 1.05E- 5.98E- -1.14E- -1.56E- -3.41E-
ADPE kg Sb eq 0 0 0 1.5E-08 0 0 0
06 08 08 07 10 08 09 07 08 09
2.45E 3.34E 7.51E 5.93E 1.85E- 2.01E 2.79E 3.38E -2.93E -5.41E -8.79E-
ADPF MJ 0 0 0 0 0 0
+02 +00 +00 +00 01 +00 +00 +00 +01 +01 01
m3 world
1.11E 2.83E- 5.25E- 9.61E- 1.57E- 6.33E- 6.36E- -3.19E- -1.51E- -4.21E- -4.53E-
WDP eq 0 0 0 0 0 0
+00 03 02 02 04 01 01 03 01 02 03
deprived
GWP = Global warming potential; ODP = Depletion potential of the stratospheric ozone layer; AP = Acidification potential of land and water; EP =
Eutrophication potential; POCP = Formation potential of tropospheric ozone photochemical oxidants; ADPE = Abiotic depletion potential for non-fossil
resources; ADPF = Abiotic depletion potential for fossil resources; WDP = Water (user) deprivation potential)
RESULTS OF THE LCA - INDICATORS TO DESCRIBE RESOURCE USE according to EN 15804+A2: 1 m² floor covering
Parameter Unit A1-A3 A4 A5 B1 B2 C1 C2 C3 C3/1 C3/2 C4 C4/1 C4/2 D D/1 D/2 D/3
3.91E 2.36E- 1.38E 3.79E 1.31E- 3.78E- 5.96E- 3.05E- -5.28E- -2.55E-
PERE MJ 0 0 0 0 0 0 -8.5E+00
+01 01 +00 +00 02 01 01 01 01 01
1.85E- -1.85E-
PERM MJ 0 0 0 0 0 0 0 0 0 0 0 0 0 0 0
01 01
3.93E 2.36E- 3.79E 1.31E- 3.78E- 5.96E- 3.05E- -5.28E- -2.55E-
PERT MJ 1.2E+00 0 0 0 0 0 0 -8.5E+00
+01 01 +00 02 01 01 01 01 01
1.87E 3.35E 7.52E 5.93E 1.86E- 5.99E 6.07E 3.38E -2.93E -5.41E -8.79E-
PENRE MJ 0 0 0 0 0 0
+02 +00 +00 +00 01 +01 +01 +00 +01 +01 01
5.79E -5.79E -5.79E
PENRM MJ 0 0 0 0 0 0 0 0 0 0 0 0 0 0
+01 +01 +01
5 Environmental Product Declaration - Fletco Carpets A/S - Woven carpet tiles, pile material polyamide 6.6 maximum total pile weight 510 g/m²
2.45E 3.35E 7.52E 5.93E 1.86E- 2.02E 2.79E 3.38E -2.93E -5.41E -8.79E-
PENRT MJ 0 0 0 0 0 0
+02 +00 +00 +00 01 +00 +00 +00 +01 +01 01
6.03E-
SM kg 0 1.81E-02 0 0 0 0 0 0 0 0 0 0 0 0 6.3E-01 0
01
RSF MJ 0 0 0 0 0 0 0 0 0 0 0 0 0 0 0 0 0
NRSF MJ 0 0 0 0 0 0 0 0 0 0 0 0 0 0 0 0 0
4.84E- 3.26E- 1.45E- 1.49E- 1.51E- 3.33E- -6.89E- -4.77E- -2.07E-
FW m3 2.6E-04 1.91E-03 0 0 0 0 0 0
02 03 05 02 02 05 03 03 04
PERE = Use of renewable primary energy excluding renewable primary energy resources used as raw materials; PERM = Use of renewable primary
energy resources used as raw materials; PERT = Total use of renewable primary energy resources; PENRE = Use of non-renewable primary energy
excluding non-renewable primary energy resources used as raw materials; PENRM = Use of non-renewable primary energy resources used as raw
materials; PENRT = Total use of non-renewable primary energy resources; SM = Use of secondary material; RSF = Use of renewable secondary fuels;
NRSF = Use of non-renewable secondary fuels; FW = Use of net fresh water
RESULTS OF THE LCA – WASTE CATEGORIES AND OUTPUT FLOWS according to EN 15804+A2:
1 m² floor covering
Parameter Unit A1-A3 A4 A5 B1 B2 C1 C2 C3 C3/1 C3/2 C4 C4/1 C4/2 D D/1 D/2 D/3
3.25E- 1.24E- 9.82E- 4.19E- 6.87E- 2.17E- 1.95E- 2.84E- -1.57E- -6.25E-
HWD kg 0 0 0 0 0 0 -4.7E-11
08 11 10 05 13 10 10 10 09 11
2.12E- 4.82E- 7.29E- 2.68E- 5.52E- 5.52E- 3.28E -1.44E- -7.31E- -4.33E-
NHWD kg 2.3E-02 0 0 0 0 0 0
01 04 03 05 01 01 +00 02 02 04
5.32E- 4.32E- 1.62E- 3.79E- 8.16E- 1.32E- -2.26E- -1.02E- -6.77E-
RWD kg 0 0 2.4E-07 0 4E-05 0 0 0
03 06 04 04 05 04 03 04 05
CRU kg 0 0 0 0 0 0 0 0 0 0 0 0 0 0 0 0 0
5.63E- 1.69E-
MFR kg 0 0 0 0 0 0 0 6.3E-01 0 0 0 0 0 0 0
02 03
MER kg 0 0 0 0 0 0 0 0 0 0 0 0 0 0 0 0 0
2.75E- 9.15E
EEE MJ 0 0 0 0 0 0 0 0 0 0 0 0 0 0 0
01 +00
4.97E- 1.66E 6.67E
EET MJ 0 0 0 0 0 0 0 0 0 0 0 0 0 0
01 +01 +01
HWD = Hazardous waste disposed; NHWD = Non-hazardous waste disposed; RWD = Radioactive waste disposed; CRU = Components for re-use;
MFR = Materials for recycling; MER = Materials for energy recovery; EEE = Exported electrical energy; EET = Exported thermal energy
RESULTS OF THE LCA – additional impact categories according to EN 15804+A2-optional:
1 m² floor covering
Parameter Unit A1-A3 A4 A5 B1 B2 C1 C2 C3 C3/1 C3/2 C4 C4/1 C4/2 D D/1 D/2 D/3
Disease 5.51E- 6.82E- 5.28E- 1.34E- 6.58E- -2.24E- -5.05E-
PM 1.6E-07 9.5E-09 0 0 0 1.5E-08 0 0 0 0
incidence 09 08 10 08 09 08 10
kBq U235 8.61E- 6.24E- 2.62E- 6.73E- 3.47E- 1.26E- 2.09E- 5.91E- -1.06E- -1.13E-
IR 0 0 0 0 0 0 0
eq 01 04 02 02 05 02 02 03 02 02
9.82E 2.35E 3.05E 3.6E- 2.07E 1.31E- 8.49E- 1.26E 2.88E -2.04E -1.22E-
ETP-fw CTUe 0 0 0 0 0 0
+01 +00 +00 03 +00 01 01 +00 +00 +01 01
3.59E- 4.75E- 1.11E- 6.26E- 2.64E- 5.65E- 6.77E- 1.48E- -9.74E- -9.72E-
HTP-c CTUh 0 0 0 0 0 0 0
09 11 10 10 12 11 11 10 11 12
9.55E- 2.09E- 2.6E- 6.16E- 1.16E- 2.17E- 2.53E- 1.18E- -3.93E- -2.39E-
HTP-nc CTUh 3E-09 0 0 0 0 0 0
08 09 11 09 10 09 09 08 09 10
SQP SQP ND ND ND ND ND 0 ND ND ND ND ND ND ND ND ND ND ND
PM = Potential incidence of disease due to PM emissions; IR = Potential Human exposure efficiency relative to U235; ETP-fw = Potential comparative
Toxic Unit for ecosystems; HTP-c = Potential comparative Toxic Unit for humans (cancerogenic); HTP-nc = Potential comparative Toxic Unit for humans
(not cancerogenic); SQP = Potential soil quality index
The SQP indicator is not given due to considerable uncertainties in the calculation.
The result figures given in module B2 refer to a period of 1 year because a reference service life is not declared. They have to be
multiplied by the assumed service life (in years) of the floor covering in the building under consideration.
Disclaimer 1 – for the indicator 'Potential Human exposure efficiency relative to U235'.
This impact category deals mainly with the eventual impact of low dose ionizing radiation on human health of the nuclear fuel cycle. It
does not consider effects due to possible nuclear accidents, occupational exposure or radioactive waste disposal in
undergroundfacilities. Potential ionizing radiation from the soil, radon and from some construction materials is also not measured by
this indicator.
Disclaimer 2 – for the indicators 'abiotic depletion potential for non-fossil resources', 'abiotic depletion potential for fossil resources',
'water (user) deprivation potential, deprivation-weighted water consumption', 'potential comparative toxic unit for ecosystems', 'potential
comparative toxic unit for humans – cancerogenic', 'Potential comparative toxic unit for humans - not cancerogenic', 'potential soil
quality index'.
The results of this environmental impact indicator shall be used with care as the uncertainties on these results are high as there is
limited experienced with the indicator.
References
EN 1307
DIN EN 1307: 2014+A1:2016+A2:2018-05: Textile floor EN 13501-1
coverings - Classification DIN EN 13501-1:2019-05: Fire classification of construction
6 Environmental Product Declaration - Fletco Carpets A/S - Woven carpet tiles, pile material polyamide 6.6 maximum total pile weight 510 g/m²
products and building elements - Part 1: Classification using Parliament, April 2011
data from reaction to fire tests
General Instructions for the IBU-EPD Program
EN 14041 General Instructions for the EPD-Program of the Institut Bauen
DIN EN 14041: 2018-05 and DIN EN 14041: 2008-05: und Umwelt e.V., The Preparation of Environmental Product
Resilient, textile and laminate floor coverings - Essential Declarations - EPDs, version 2.0, Institut Bauen und Umwelt
characteristics e.V., Berlin, January 2021, www.ibu-epd.de
EN 15804 BBSR
DIN EN 15804:2012+A2:2019 + AC:2021, Sustainability of Bundesinstitut für Bau-, Stadt- und Raumforschung (BBSR) im
construction works — Environmental Product Declarations — Bundesamt für Bauwesen und Raumordnung (BBR), Bonn
Core rules for the product category of construction products
BNB, Nutzungsdauer von Bauteilen
EN 16810 Bewertungssystem Nachhaltiges Bauen (BNB), Nutzungsdauer
DIN EN 16810: 2017-08: Resilient, textile and laminate floor von Bauteilen, Bundesministerium des Inneren, für Bau und
coverings – Environmental product declarations – Product Heimat, 24.02.2017
category rules
ECHA candidate list
ISO 10874 Candidate List of substances of very high concern (SVHCs) for
DIN EN ISO 10874: 2012+A1:2021-04: Resilient, textile and authorisation, last update 23.01.2024, European Chemicals
laminate floor coverings - Classification Agency (ECHA), Helsinki, Finland
ISO 14025 Sphera MLC and LCA FE
DIN EN /ISO 14025:2011-10/, Environmental labels and Software-System and Database for Life Cycle Engineering,
declarations — Type III environmental declarations — Sphera, Leinfelden-Echterdingen, 2023-2
Principles and procedures
PCR Part A
ISO 14040 Product Category Rules for Building-Related Products and
DIN EN ISO 14040:2006+A1:2020 Environmental Services Part A: Calculation Rules for the Life Cycle
management - Life cycle assessment - Principles and Assessment and Requirements on the Project Report according
framework to EN 15804+A2:2019, V1.3, Berlin: Institut Bauen und Umwelt
e.V. (IBU), August 2022
ISO 14044
DIN EN ISO 14044:2006+A1:2018+A2:2020 Environmental PCR Part B
management - Life cycle assessment - Requirements and Product Category Rules for Building-Related Products and
guidelines Services Part B: Requirements on the EPD for floor coverings,
V1.4, Berlin: Institut Bauen und Umwelt e.V. (IBU), June 2023
ISO 15686
ISO 15686: Buildings and constructed assets - Service life PRODIS
planning Product Information System (PRODIS) of the European Carpet
ISO 15686-1: 2011-05: Part 1: General principles and Industry, Gemeinschaft umweltfreundlicher Teppichboden e.V
framework (GUT) and European Carpet and Rug Association (ECRA),
ISO 15686-2: 2012-05: Part 2: Service life prediction http://www.pro-dis.info
procedures
ISO 15686-7: 2017-04: Part 7: Performance evaluation for REACH
feedback of service life data from practice Regulation (EC) No 1907/2006 of the European Parliament and
ISO 15686-8: 2008-06: Part 8: Reference service life and of the Council of 18 December 2006 concerning the
service- Registration, Evaluation, Authorisation and Restriction of
life estimation Chemicals (REACH), June 2017
Regulation (EU) No. 305/2011 VDZ e.V.
Regulation No. 305/2011 Construction Products Regulation Association of German Cement Works, Ed. Environmental Data
(CPR) of the European Council and of the European of the German Cement Industry 2020
7 Environmental Product Declaration - Fletco Carpets A/S - Woven carpet tiles, pile material polyamide 6.6 maximum total pile weight 510 g/m²
Publisher
Institut Bauen und Umwelt e.V. +49 (0)30 3087748- 0
Hegelplatz 1 info@ibu-epd.com
10117 Berlin www.ibu-epd.com
Germany
Programme holder
Institut Bauen und Umwelt e.V. +49 (0)30 3087748- 0
Hegelplatz 1 info@ibu-epd.com
10117 Berlin www.ibu-epd.com
Germany
Author of the Life Cycle Assessment
Gemeinschaft umweltfreundlicher Teppichboden +49 (0)241 96843 410
(GUT) e.V. mail@gut-ev.de
Schönebergstraße 2 www.gut-ev.org
52068 Aachen
Germany
Owner of the Declaration
Fletco Carpets A/S +45 (0)96 60 30 00
Mads Clausens Vej 2 fletco@fletco.dk
7441 Bording www.fletcocarpets.com
Denmark
8 Environmental Product Declaration - Fletco Carpets A/S - Woven carpet tiles, pile material polyamide 6.6 maximum total pile weight 510 g/m²
