ENVIRONMENTAL-PRODUCT DECLARATION
as per ISO 14025 and EN 15804+A2
Owner of the Declaration GLAPOR Werk Mitterteich GmbH
Publisher Institut Bauen und Umwelt e.V. (IBU)
Programme holder Institut Bauen und Umwelt e.V. (IBU)
Declaration number EPD-GLP-20230178-CBA2-EN
Issue date 09.10.2023
Valid to 08.10.2028
GLAPOR cellular glass gravel
GLAPOR Werk Mitterteich GmbH
www.ibu-epd.com | https://epd-online.com
General Information
GLAPOR Werk Mitterteich GmbH GLAPOR cellular glass gravel
Programme holder Owner of the declaration
IBU – Institut Bauen und Umwelt e.V. GLAPOR Werk Mitterteich GmbH
Hegelplatz 1 Hüblteichstraße 17
10117 Berlin 95666 Mitterteich
Germany Germany
Declaration number Declared product / declared unit
EPD-GLP-20230178-CBA2-EN GLAPOR cellular glass gravel / 1 m3 at 140 kg/m3 (compacted)
This declaration is based on the product category rules: Scope:
Mineral insulating materials, 01.08.2021 The EPD represents cellular glass gravel produced at the GLAPOR
(PCR checked and approved by the SVR) production site at Mitterteich/GER.
The owner of the declaration shall be liable for the underlying information
and evidence; the IBU shall not be liable with respect to manufacturer
Issue date information, life cycle assessment data and evidences.
09.10.2023
The EPD was created according to the specifications of EN 15804+A2. In
the following, the standard will be simplified as EN 15804 bezeichnet.
Valid to
Verification
08.10.2028
The standard EN 15804 serves as the core PCR
Independent verification of the declaration and data according to ISO
14025:2011
internally X externally
Dipl.-Ing Hans Peters
(chairman of Institut Bauen und Umwelt e.V.)
Florian Pronold Angela Schindler,
(Managing Director Institut Bauen und Umwelt e.V.) (Independent verifier)
1 Environmental-Product Declaration - GLAPOR Werk Mitterteich GmbH - GLAPOR cellular glass gravel
Product
GLAPOR insulation gravel is a load bearing filling of foamed
Product description/Product definition recycled glass, for use as thermal insulation
GLAPOR CELLULAR glass gravel is an insulating and light GLAPOR light gravel is a light aggregate for unbound and
construction material for the construction industry made of 100 bound use.
% recycled glass. It combines the structural-physical properties GLAPOR filling gravel is a light aggregate, which can be used
of glass with the insulation properties of a closed-cell structure. as filling material.
GLAPOR cellular glass gravel can be used as a load bearing
and insulating bulk under every house or construction. Technical Data
Technical data
Lifetime characteristics:
Name Value Unit
• high compression strength
100 -
• made of 100% recycled glass Bulk density (EN 1097-3) kg/m³
120
• demountable, urban mining compatible
Grain size (EN 933-1) 16 - 63 mm
This EPD is valid for the GLAPOR cellular glass gravel: Thermal conductivity declared value (EN
0,083 W/mK
13167)
Building market Rated value of compression strength fcd (EN
≥ 225 kPa
SG270 F 100 – 120 kg/m³ 826)
SG370 T 100 – 125 kg/m³ Compaction ratio 1,3:1
SG600 100 – 120 kg/m³
Performance data of the product in accordance with the
SG600 P 100 – 120 kg/m³
Declaration of Performance with respect to its Essential
SG600 E 100 – 120 kg/m³
Characteristics according to EN 13167:2012+A1:2015, Thermal
SG600 T 100 – 125 kg/m³
insulation products for buildings - Factory made cellular glass
SG800 135 – 170 kg/m³
(CG) products - Specification.
SG800 P 150 – 170 kg/m³
SG800 T 140 – 170 kg/m³
Base materials/Ancillary materials
SG800 E 150 – 170 kg/m³
GLAPOR cellular glass is composed of:
Fullschotter / Filling Gravel / Granulate • 97 % of recycled glass
FSA10 130 – 180 kg/m³ • 3 % of sodium silicate ("water glass")
GFS 50 100 – 130 kg/m³ In addition, minor quantities of glycerine and kaolin are used.
GFS 100 100 – 130 kg/m³
The product does not contain substances listed in the ECHA
Gravel for street construction (lowering weight) Candidate List of Substances of Very High Concern for
SG 2000 FGSV 135 – 170 kg/m³ Authorisation (accessed 5.11.2022) exceeding the limit value of
0.1% for registration by the European Chemicals Agency.
For the placing on the market of the product in the European
Environment and health during use
Union/European Free Trade Association (EU/EFTA) (with the
exception of Switzerland) Regulation (EU) No. 305/2011 (CPR)
Reference service life
applies. The product needs a Declaration of Performance
If installed according to the manufacturer's instructions, the
taking into consideration EN 13167:2012+A1:2015, Thermal
service life of the insulation material will reach the service life of
insulation products for buildings. Factory made cellular glass
the building, i.e. 100 years or more.
(CG) products and the CE-marking.
Application According to the table on expected service lives for the German
BNB scheme BBSR 2017, a service life of ≥ 50 years can be
assumed for all relevant applications.
LCA: Calculation rules
Type of EPD: "cradle to gate with options, modules C1–C3, and
Declared Unit module D (A1–A3, C, D and additional modules. The additional
The declaration is valid for 1 m3 of GLAPOR cellular glass modules may be A4 and/or A5 and/or B1–B7)".
gravel SG 800 with a density of 138,5 kg/m3 (non-compacted).
The system boundary of modules A1–A3 encompasses all
Declared unit
processes related to the production of cellular glass gravel as a
Name Value Unit
co-product of the production of cellular glass insulation boards.
Gross density (after compaction) 138.5 kg/m3 The system boundary for the recycled glass is assumed to be
Declared unit 1 m³ after the sorting of the glass cullets that are to be recycled.
Within the system boundary of A1–A3 are considered:
The selected product SG 800 represents the product with the
highest production volume as the "typical product". The • grinding of recycled glass cullets
declared values can be extrapolated to any product and • production of all ancillary materials
thickness via the respective area weight. • electricity production
• heat generation for the production process
System boundary • production of packaging material
2 Environmental-Product Declaration - GLAPOR Werk Mitterteich GmbH - GLAPOR cellular glass gravel
• all transport, including transport of glass cullets to the Module D/1 contains the benefits of replacing natural crushed
external grinding and transport of inputs to the gravel calculated for the net flow calculated as the difference
production site. between the output of recycled cellular glass and the input of
The process does not generate waste water. glass cullet.
The production process of cellular glass insulation boards
generates about 30 % of production waste that is used for the Scenario 2: landfilling:
production of cellular glass gravel. For this product, an
economic allocation is applied. Module C2/2 contains a default transport scenario (50 km by
No other waste is generated in significant quantities. lorry) of the cellular glass gravel from the deconstruction site to
an inert material landfill.
Module A4 contains the average transport scenario from the
production site to the construction site.
Module C4/2 contains the landfilling of the cellular glass gravel.
Module A5 contains the energy needed for the compacting of
the cellular glass gravel on the construction site. The disposal Module D/2 does not contain any loads and benefits.
of reusable big bags as transport packaging is disregarded.
Geographic Representativeness
Module C1 contains the energy needed for de-construction. Land or region, in which the declared product system is
After de-construction, 2 scenarios are declared: manufactured, used or handled at the end of the product´s
lifespan: Germany
Scenario 1: reuse as cellular glass gravel
Comparability
Module C2/1 contains a default transport scenario (350 km by
Basically, a comparison or an evaluation of EPD data is only
lorry) of the cellular glass gravel from the deconstruction site to
possible if all the data sets to be compared were created
the next construction site; this system boundary is set in a
according to EN 15804 and the building context, respectively
conservative way.
the product-specific characteristics of performance, are taken
into account.
Module C3/1 does not contain any impacts as a direct
The database ecoinvent 3.9.1 (system model "cut-off by
replacement with primary gravel is assumed.
classification") was used as background database.
LCA: Scenarios and additional technical information
Characteristic product properties Name Value Unit
Information on biogenic carbon
Life Span (according to BBSR) ≥ 50 a
100 years and
Life Span according to the beyond, depending
a
Information on biogenic carbon content at factory gate manufacturer on the service life of
Name ValueUnit the building
kg Declared product properties (at the compliance with EN
Biogenic carbon content in product 0 -
C gate) and finishes 13167
Biogenic carbon content in accompanying kg Design application parameters (if
0
packaging C instructed by the manufacturer), according to the
including the references to the instructions by the -
appropriate practices and manufacturer
Transport to construction site (A4)
application codes
installation according
A default distance of 350 km is assumed for the transport from An assumed quality of work, when
to assembly
the production to the construction site. Capacity utilisation and installed in accordance with the -
instructions and state
fuel consumption are taken from the ecoinvent dataset for an manufacturer’s instructions
of the art.
average transport by lorry in Europe and have not been
modified. Outdoor environment, (for outdoor
applications), e.g. weathering,
Construction (A5) pollutants, UV and wind exposure, not applicable -
building orientation, shading,
For the compacting of the gravel from 39 cm to 30 cm, petrol is temperature
used in a compacting device (4 l/h and 200 m2/h). Indoor environment (for indoor
usual conditions in
applications), e.g. temperature, -
structural engieering
The use of multi-way pallets and reusable big bags has not moisture, chemical exposure
been taken into account as packaging material. Usage conditions, e.g. frequency of
not applicalbe -
Service life use, mechanical exposure
Maintenance e.g. required
no maintenance
frequency, type and quality and -
required
replacement of components
C1-C4 End-of-life scenario
In Module C1, the petrol consumption for deconstructing the
gravel is inventoried, assuming the same amount of fuel as for
3 Environmental-Product Declaration - GLAPOR Werk Mitterteich GmbH - GLAPOR cellular glass gravel
the compacting. After de-construction, 2 scenarios are lorry) of the cellular glass gravel from the deconstruction site to
declared: the inert material landfill.
Scenario 1: re-use as gravel Module C4/2 contains the landfilling of the cellular glass gravel
in an inert material landfill.
Module C2/1 contains a default transport scenario (350 km by
lorry) of the cellular glass gravel from the deconstruction site to D Benefits and burdens beyond system boundary
the site of re-use (this system boundary is set in a conservative
way). Module D/1 contains the benefits of replacing natural crushed
gravel, calculated for the net flow calculated as the difference
Module C3/1 does not contain any impact from re-use. between the output of recycled cellular glass and the input of
glass cullet.
Scenario 2: landfilling
Module D/2 does not contain any benefits and burdens beyond
Module C2/2 contains a default transport scenario (50 km by the system boundary.
4 Environmental-Product Declaration - GLAPOR Werk Mitterteich GmbH - GLAPOR cellular glass gravel
LCA: Results
For the calculation of the impact assessment, EN 15804:2012+A2:2019+AC:2021 based on EF 3.1 has been used.
DESCRIPTION OF THE SYSTEM BOUNDARY (X = INCLUDED IN LCA; ND = MODULE OR INDICATOR NOT DECLARED; MNR =
MODULE NOT RELEVANT)
BENEFITS
AND LOADS
CONSTRUCTION
BEYOND
PRODUCT STAGE PROCESS USE STAGE END OF LIFE STAGE
THE SYSTEM
STAGE
BOUNDARIE
S
la ire ta m w a Ry lp p u s tro p s n a rT g n iru tc a fu n a M e h t m o rf tro p s n a rTe tis e h t o t e ta g y lb m e s s A e s U e c n a n e tn ia M ria p e R tn e m e c a lp e R tn e m h s ib ru fe R y g re n e la n o ita re p Oe s u re ta w la n o ita re p Oe s u n o itc u rts n o c -e Dn o itilo m e d tro p s n a rT g n is s e c o rp e ts a W la s o p s iD -e s u e R-y re v o c e R-g n ilc y c e Rla itn e to p
A1 A2 A3 A4 A5 B1 B2 B3 B4 B5 B6 B7 C1 C2 C3 C4 D
X X X X X MND MND MNR MNR MNR MND MND X X X X X
RESULTS OF THE LCA - ENVIRONMENTAL IMPACT according to EN 15804+A2: GLAPOR cellular glass gravel SG 800 / per m³
(138,5 kg/m³)
Parameter Unit A1-A3 A4 A5 C1 C2/1 C2/2 C3/1 C4/2 D/1 D/2
GWP-total kg CO 2 eq 3.87E+01 7.17E+00 2.44E-01 2.44E-01 7.17E+00 1.02E+00 0 8.33E-01 -2.79E-02 0
GWP-fossil kg CO 2 eq 3.87E+01 7.16E+00 2.44E-01 2.44E-01 7.16E+00 1.02E+00 0 8.31E-01 -2.68E-02 0
GWP-
biogenic kg CO 2 eq 1.18E-02 6.5E-03 2.83E-05 2.83E-05 6.5E-03 9.29E-04 0 2.68E-03 -1.06E-03 0
GWP-luluc kg CO 2 eq 7.35E-03 3.41E-03 1.38E-05 1.38E-05 3.41E-03 4.88E-04 0 1.55E-04 -1.93E-05 0
ODP kg CFC11 eq 1.24E-06 1.52E-07 2.9E-09 2.9E-09 1.52E-07 2.17E-08 0 2.72E-08 -4.29E-10 0
AP mol H+ eq 8.19E-02 2.29E-02 9.89E-04 9.89E-04 2.29E-02 3.27E-03 0 5.06E-03 -2.16E-04 0
EP-
kg P eq 7.13E-04 5.7E-05 4.12E-07 4.12E-07 5.7E-05 8.14E-06 0 4.49E-06 -6.55E-07 0
freshwater
EP-marine kg N eq 2.42E-02 7.77E-03 4.12E-04 4.12E-04 7.77E-03 1.11E-03 0 2.2E-03 -6.29E-05 0
EP-terrestrial mol N eq 2.32E-01 8.3E-02 4.47E-03 4.47E-03 8.3E-02 1.19E-02 0 2.37E-02 -8.54E-04 0
kg NMVOC
POCP 8.04E-02 3.48E-02 3.34E-03 3.34E-03 3.48E-02 4.97E-03 0 9.38E-03 -2.18E-04 0
eq
ADPE kg Sb eq 1.11E-04 2.14E-05 4.12E-08 4.12E-08 2.14E-05 3.06E-06 0 8.25E-07 -3.62E-07 0
ADPF MJ 5.32E+02 1E+02 2.48E+00 2.48E+00 1E+02 1.43E+01 0 1.99E+01 -3.89E-01 0
m3 world eq
WDP 3.08E+00 4.47E-01 4.01E-03 4.01E-03 4.47E-01 6.38E-02 0 7.25E-02 -6.57E-03 0
deprived
GWP = Global warming potential; ODP = Depletion potential of the stratospheric ozone layer; AP = Acidification potential of land and water; EP =
Eutrophication potential; POCP = Formation potential of tropospheric ozone photochemical oxidants; ADPE = Abiotic depletion potential for non-fossil
resources; ADPF = Abiotic depletion potential for fossil resources; WDP = Water (user) deprivation potential)
RESULTS OF THE LCA - INDICATORS TO DESCRIBE RESOURCE USE according to EN 15804+A2: GLAPOR cellular glass
gravel SG 800 / per m³ (138,5 kg/m³)
Parameter Unit A1-A3 A4 A5 C1 C2/1 C2/2 C3/1 C4/2 D/1 D/2
PERE MJ 1.7E+01 1.55E+00 6.87E-03 6.87E-03 1.55E+00 2.22E-01 0 3.85E-01 -1.23E-01 0
PERM MJ 0 0 0 0 0 0 0 0 0 0
PERT MJ 1.7E+01 1.55E+00 6.87E-03 6.87E-03 1.55E+00 2.22E-01 0 3.85E-01 -1.23E-01 0
PENRE MJ 5.32E+02 1E+02 2.49E+00 2.49E+00 1E+02 1.43E+01 0 1.99E+01 -3.89E-01 0
PENRM MJ 0 0 0 0 0 0 0 0 0 0
PENRT MJ 5.32E+02 1E+02 2.49E+00 2.49E+00 1E+02 1.43E+01 0 1.99E+01 -3.89E-01 0
SM kg 1.31E+02 0 0 0 0 0 0 0 7.4E+00 0
RSF MJ 0 0 0 0 0 0 0 0 0 0
NRSF MJ 0 0 0 0 0 0 0 0 0 0
FW m3 1.46E-01 2.74E-02 2.6E-04 2.6E-04 2.74E-02 3.91E-03 0 2.7E-03 -2.8E-03 0
PERE = Use of renewable primary energy excluding renewable primary energy resources used as raw materials; PERM = Use of renewable primary
energy resources used as raw materials; PERT = Total use of renewable primary energy resources; PENRE = Use of non-renewable primary energy
excluding non-renewable primary energy resources used as raw materials; PENRM = Use of non-renewable primary energy resources used as raw
materials; PENRT = Total use of non-renewable primary energy resources; SM = Use of secondary material; RSF = Use of renewable secondary fuels;
NRSF = Use of non-renewable secondary fuels; FW = Use of net fresh water
RESULTS OF THE LCA – WASTE CATEGORIES AND OUTPUT FLOWS according to EN 15804+A2:
GLAPOR cellular glass gravel SG 800 / per m³ (138,5 kg/m³)
Parameter Unit A1-A3 A4 A5 C1 C2/1 C2/2 C3/1 C4/2 D/1 D/2
HWD kg 1.97E-03 6.31E-04 2.25E-05 2.25E-05 6.31E-04 9.01E-05 0 9.73E-05 -2.56E-06 0
NHWD kg 4.28E+00 6.58E+00 2.1E-03 2.1E-03 6.58E+00 9.41E-01 0 1.38E+02 -7.24E-03 0
RWD kg 1.04E-03 5.82E-05 2.52E-07 2.52E-07 5.82E-05 8.31E-06 0 7.68E-06 -2.65E-06 0
5 Environmental-Product Declaration - GLAPOR Werk Mitterteich GmbH - GLAPOR cellular glass gravel
CRU kg 0 0 0 0 0 0 1.39E+02 0 0 0
MFR kg 1.36E-03 0 0 0 0 0 0 0 0 0
MER kg 0 0 0 0 0 0 0 0 0 0
EEE MJ 0 0 0 0 0 0 0 0 0 0
EET MJ 0 0 0 0 0 0 0 0 0 0
HWD = Hazardous waste disposed; NHWD = Non-hazardous waste disposed; RWD = Radioactive waste disposed; CRU = Components for re-use;
MFR = Materials for recycling; MER = Materials for energy recovery; EEE = Exported electrical energy; EET = Exported thermal energy
RESULTS OF THE LCA – additional impact categories according to EN 15804+A2-optional:
GLAPOR cellular glass gravel SG 800 / per m³ (138,5 kg/m³)
Parameter Unit A1-A3 A4 A5 C1 C2/1 C2/2 C3/1 C4/2 D/1 D/2
Disease
PM 7.69E-07 6.05E-07 2.9E-09 2.9E-09 6.05E-07 8.65E-08 0 1.28E-07 -4.71E-09 0
incidence
IR kBq U235 eq 5E-01 5.15E-02 3.33E-04 3.33E-04 5.15E-02 7.36E-03 0 7.79E-03 -2.67E-03 0
ETP-fw CTUe 1.33E+02 5.29E+01 1.3E+00 1.3E+00 5.29E+01 7.56E+00 0 8.84E+00 -2.12E-01 0
HTP-c CTUh 9.9E-09 3.12E-09 9.64E-11 9.64E-11 3.12E-09 4.46E-10 0 2.66E-10 -5.08E-11 0
HTP-nc CTUh 2.75E-07 9.28E-08 4.47E-08 4.47E-08 9.28E-08 1.33E-08 0 6.56E-09 -6.28E-10 0
SQP SQP 1.1E+02 7.75E+01 1.54E-01 1.54E-01 7.75E+01 1.11E+01 0 4.11E+01 -7.68E-01 0
PM = Potential incidence of disease due to PM emissions; IR = Potential Human exposure efficiency relative to U235; ETP-fw = Potential comparative
Toxic Unit for ecosystems; HTP-c = Potential comparative Toxic Unit for humans (cancerogenic); HTP-nc = Potential comparative Toxic Unit for humans
(not cancerogenic); SQP = Potential soil quality index
Disclaimer 1 – for the indicator “Potential Human exposure efficiency relative to U235”. This impact category deals mainly with the
eventual impact of low dose ionizing radiation on human health of the nuclear fuel cycle. It does not consider effects due to possible
nuclear accidents, occupational exposure nor due to radioactive waste disposal in underground facilities. Potential ionizing radiation
from the soil, from radon and from some construction materials is also not measured by this indicator.
Disclaimer 2 – for the indicators “abiotic depletion potential for non-fossil resources”, “abiotic depletion potential for fossil resources”,
“water (user) deprivation potential, deprivation-weighted water consumption”, “potential comparative toxic unit for ecosystems”,
“potential comparative toxic unit for humans – cancerogenic”, “Potential comparative toxic unit for humans - not cancerogenic”,
“potential soil quality index”. The results of this environmental impact indicator shall be used with care as the uncertainties on these
results are high or as there is limited experienced with the indicator.
References
Product category rules of IBU density and voids.
IBU (2021) EN 1602
IBU (2021): General Instructions for the EPD Programme of the DIN EN 1602:2013-05, Thermal insulating products for building
Institut Bauen & Umwelt e.V. (General Instructions for the IBU applications – Determination of the apparent density.
EPD Programme). Version 2.0, Institut Bauen & Umwelt, Berlin.
EN 13167+A1
IBU (2022) EN 13167:2012+A1:2015, Thermal insulation products for
IBU (2022): PCR Part A: Calculation rules for the life cycle buildings – Factory made cellular glass (CG) products –
assessment and requirements on the project report according Specification.
to EN 15804+A2. Version 1.3., Institut Bauen & Umwelt, Berlin.
EN 13501-1
IBU (2023) DIN EN 13501-1:2010-01, Fire classification of construction
IBU (2023): PCR Part B: Requirements on the EPD for mineral products and building elements – Part 1: Classification using
insulation materials. Version 2023/04, Institut Bauen & Umwelt, data from reaction to fire tests.
Berlin
EN 15804
Standards and legal documents EN 15804:2012+A2:2019+AC:2021, Sustainability of
construction works – Environmental product declarations –
DIN 4108-10 Core rules for the product category construction products.
DIN 4108-10:2021-11, Thermal insulation and energy economy
in buildings – Part 10: Application-related requirements for ISO 14025
thermal insulation materials – Factory made products. ISO 14025:2006-07, Environmental labels and declarations –
Type III Environmental declarations – Principles and
EN 826 procedures.
DIN EN 826:2013-05, Thermal insulating products for building
applications – Determination of compression behaviour. ISO 14044
EN ISO 14044:2006-07, Environmental management – Life
EN 933-1 cycle assessment – Requirements and guidance (ISO
DIN EN 933-1:2012-03, Tests for geometrical properties of 14044:2006).
aggregates – Part 1: Determination of particle size distribution –
Sieving method. ISO 15686
ISO 15686:1,-2, -7 and -8. Service life planning (various parts)
EN 1097-3
DIN EN 1097-3:1998-06, Tests for mechanical and physical Additional references
properties of aggregates – Part 3: Determination of loose bulk
6 Environmental-Product Declaration - GLAPOR Werk Mitterteich GmbH - GLAPOR cellular glass gravel
BBSR 2011 candidate-list.
BBSR (2011): Nutzungsdauer von Bauteilen in
Lebenszyklusanalysen nach Bewertungssystem Nachhaltiges ecoinvent 3.9.1
Bauen (BNB). Version vom 3.11.2011, Bundesinstitut für Bau-, Life cycle inventory database ecoinvent v.3.9.1, 12-2022.
Stadt- und Raumforschung, Berlin.
Regulation (EU) Nr. 305/2011(CPR)
ECHA candidate list REGULATION (EU) No 305/2011 OF THE EUROPEAN
The candidate list of substances of very high concern, PARLIAMENT AND OF THE COUNCIL of 9 March 2011 laying
European Chemicals Agency, Helsinki. Available at: down harmonised conditions for the marketing of construction
https://echa.europa.eu/nl/-/four-newsubstances-added-to-the products and repealing Council Directive 89/106/EEC.
7 Environmental-Product Declaration - GLAPOR Werk Mitterteich GmbH - GLAPOR cellular glass gravel
Publisher
Institut Bauen und Umwelt e.V. +49 (0)30 3087748- 0
Hegelplatz 1 info@ibu-epd.com
10117 Berlin www.ibu-epd.com
Germany
Programme holder
Institut Bauen und Umwelt e.V. +49 (0)30 3087748- 0
Hegelplatz 1 info@ibu-epd.com
10117 Berlin www.ibu-epd.com
Germany
Author of the Life Cycle Assessment
Dr. Frank Werner - Umwelt & Entwicklung + 41 (0)44 241 39 06
Kammelenbergstrasse 30 frank@frankwerner.ch
9011 St. Gallen http://www.frankwerner.ch/
Switzerland
Owner of the Declaration
GLAPOR Werk Mitterteich GmbH +49 9633 4007690
Hüblteichstraße 17 info@glapor.de
95666 Mitterteich www.glapor.de
Germany
8 Environmental-Product Declaration - GLAPOR Werk Mitterteich GmbH - GLAPOR cellular glass gravel
