DAPHabitat System Environmental Product Declarat ion
www.daphabitat.pt [according to ISO 14025, EN 15804:2012+A2:2019 and EN 15942]
Declaration number: DAP 009:2024
GLAZED VITRIFIED TILES
ISSUE DATE: 25/09/2024 VALID UNTIL: 24/09/2029
PAVIGRÉS CERÂMICAS, S.A.
Version 1.4. Ed. Março 2024
Sistema DAPHabitat
i
INDEX
1. GENERAL INFORMATION ................................................................................................................. 1
1.1. The DAPHAbitat System .............................................................................................................................. 1
1.2. EPD owner ................................................................................................................................................... 1
1.3. Information concerning the EPD ................................................................................................................. 3
1.4. Demonstration of the verification .............................................................................................................. 3
1.5. EPD Registration .......................................................................................................................................... 3
1.6. PCR (product category rules) basic model .................................................................................................. 4
1.7. Relevant c-PCR (Complementary product category rules)* ....................................................................... 4
1.8. Information concerning the product/product class ................................................................................... 5
1.9. Calculation rules of the LCA ........................................................................................................................ 7
1.10. Use of average environmental performance ............................................................................................. 7
1.11. Technical information for Reference Service Life (RSL) ............................................................................. 8
1.12. Flow diagram of input and output of the processes .................................................................................. 9
2. CORE ENVIRONMENTAL IMPACT INDICATORS............................................................................. 13
2.1. Description of the system boundaries ...................................................................................................... 13
2.1.1. Justification for the exemption to declare modules C1, C2, C3, C4 and D............................................... 14
2.2. Core environmental impact indicators ..................................................................................................... 15
2.3. Additional environmental impact indicators ........................................................................................... 17
2.4. Indicators describing resource use ........................................................................................................... 18
2.5. Other environmental information describing different waste categories .............................................. 20
2.6. Environmental information describing output flows ............................................................................... 21
2.7. Information describing the biogenic carbon content at the factory gate ............................................... 22
3. SCENARIOS AND ADDITIONAL TECHNICAL INFORMATION .......................................................... 22
3.1. A4 Transport to the building site – Construction process stage .............................................................. 22
3.2. A5 Installation of the product in the building – Construction process stage .......................................... 22
3.3. B1 Use stage .............................................................................................................................................. 23
3.4. B2 Maintenance ........................................................................................................................................ 23
3.5. B3 Repair ................................................................................................................................................... 23
3.6. B4 Replacement ........................................................................................................................................ 23
3.7. B5 Rehabilitation ....................................................................................................................................... 24
3.8. B6 Use of energy (operational) ................................................................................................................. 24
3.9. B7 Use of water (operational) ................................................................................................................... 24
3.10. C1 De-construction, demolition – End of life of the product ................................................................... 24
3.11. C2 Transport – End of life of the product ................................................................................................. 24
3.12. C3 Waste processing for reuse, recovery and/or recycling – End of life of the product ......................... 24
3.13. C4 Disposal – End of life of the product.................................................................................................... 24
3.14. Scenario and technical information for module D ................................................................................... 24
Sistema DAPHabitat
ii
3.15. Additional information on release of dangerous substances to indoor air, soil, and water during the
use stage ................................................................................................................................................................. 25
4. REFERENCES ................................................................................................................................... 26
Sistema DAPHabitat
iii
1. GENERAL INFORMATION
1.1. The DAPHAbitat System
Associação Plataforma para a Construção Sustentável
Program operator: www.clusterhabitat.pt
geral@clusterhabitat.pt
Departamento Engenharia Civil
Address:
Universidade de Aveiro
3810-193 Aveiro
Email address: deptecnico@clusterhabitat.pt
Telephone number: (+351) 234 401576
www.daphabitat.pt
Website:
Logo
1.2. EPD owner
Name of the owner: Pavigrés Cerâmicas, S. A.
Pavigrés Cerâmicas, S.A. – Unidade Fabril Pavigrés, Av. Alto das Domingas, 3780-244 –
Production site:
Aguim
Address (head office): Pavigrés Cerâmicas, S.A., Av. Alto das Domingas, 3780-244 – Aguim
Telephone: (+351) 231 510 600
E-mail: geral@pavigres.com
Website: www.pavigres.com
Logo:
Information concerning the ISO 9001:2015 – Quality Management Systems
applicable management
ISO 14001:2015 – Environmental Management Systems
Systems:
Specific aspects regarding
the production: CAE Rev.3 n.º 23312 – Manufacture of tiles, mosaics and ceramic plates
PAVIGRÉS CERÂMICAS, S.A. is:
Mission:
Create and produce flooring and ceramic tiles that reinforce PAVIGRES prestige and trust in
the global market, ensuring the Group's sustainability and development.
Organization’s
Policy:
environmental policy:
PAVIGRÉS CERÂMICAS, S.A., assumes, as a fundamental vector for its success, the
permanent focus on the Customer, demonstrated by the constant concern to anticipate
and meet market expectations. This company presents global and integrated ceramic
coating and flooring solutions, with products that stand out in the market due to their
recognized quality and aesthetic value.
This Policy is aligned and developed in the following aspects:
DAPHabitat System 1
Promote and encourage the continuous improvement of its Management System, to
guarantee high levels of performance of its processes, products and services, with a view to
meeting and exceeding the needs and expectations of customers, shareholders and other
relevant stakeholders;
Provide the company with human resources, developing the skills of its employees,
encouraging initiative, productivity and a responsible attitude in improving processes and
procedures;
Comply with applicable compliance obligations, namely legal, regulatory, normative and
others that PAVIGRÉS endorses as applicable;
Protect the Environment by promoting the prevention of pollution through the
management of the consumption of natural water and energy resources and the
implementation of good practices, namely, further the recovery of waste over its
elimination, whenever possible, to allow continuous improvement of the environmental
performance;
Provide the necessary resources and means to comply with the established Strategic
Guidelines, creating conditions for possible investments in new projects focused on
satisfying relevant stakeholders, to promote the financial consolidation of PAVIGRÉS.
The Management System Policy is thus adopted by PAVIGRÉS with LOYALTY, RIGOR, AND
COMMITMENT, being communicated to all employees and disclosed to other interested
parties, as appropriate.
DAPHabitat System 2
1.3. Information concerning the EPD
Authors: 1. Centro Tecnológico da Cerâmica e do Vidro
2. PAVIGRÉS CERÂMICAS, S.A.
Contact of the authors: 1. CTCV materials: habitat | iParque – Parque Tecnológico de Coimbra – Lote 6 |
3040-540 Antanhol – Portugal
(T) +351 239 499 200
Marisa Almeida: marisa@ctcv.pt
2. Pavigrés Cerâmicas, S. A., Av. Alto das Domingas, 3780-244 – Aguim
(T) +351 231 510 600
e-mail: ritatovim@pavigres.com
Issue date: 25/09/2024
Registration date:
27/09/2024
Registration number: DAP 009:2024
Valid until:
24/09/2029
Representativity of the EPD
(location, manufacturer, EPD of one (1) product class, produced in one (1) industrial unit, belonging to one (1) single
producer (Pavigrés Cerâmicas, S.A.)
group of manufacturers):
Where to consult
www.pavigres.com
explanatory material:
Type of EPD: EPD from Cradle-to-grave and module D (A1-D)
1.4. Demonstration of the verification
External independent verification, according to the standard ISO 14025:2010 and EN 15804:2012+A2:2019
Certification Body Verifier
(CERTIF – Associação para a Certificação) (Ricardo Mateus)
1.5. EPD Registration
Programme operator
(Plataforma para a Construção Sustentável)
DAPHabitat System 3
1.6. PCR (product category rules) basic model
Name: PCR: Basic module for construction products and services
Issue date: Edition August 2023
Number of registration on the RCP-mb001
database:
Version: Version 2.3
Identification and contact of the Marisa Almeida | marisa@ctcv.pt
coordinator (s): Luís Arroja | arroja@ua.pt
José Dinis Silvestre | jose.silvestre@ist.utl.pt
Marisa Almeida | marisa@ctcv.pt
Identification and contact of the
Luís Arroja | arroja@ua.pt
authors:
José Silvestre | jds@civil.ist.utl.pt
Fausto Freire
Cristina Rocha
Ana Paula Duarte
Ana Cláudia Dias
Helena Gervásio
Victor Ferreira
Ricardo Mateus
António Baio Dias
Composition of the Sectorial Panel: -
Consultation period: 18/11/2015 - 18/01/2016
Valid until: 01/06/2027
CEN standard EN 15804 serves as the core Product Category Rules (PCR)
1.7. Relevant c-PCR (Complementary product category rules)*
Name: 1. RCP: Floor covering
2. RCP: Wall covering
3. EN 17160:2019 – Product Category Rules for Ceramic Tiles
Issue date: 1. 10/02/2014
2. 10/02/201a
3. 27/02/2019, in force since 15/04/2019
Number of registration on the 1. RCP001:2014
database: 2. RCP002:2014
3. --
Version: 1. Version 1.2 (June 2022)
2. Version 1.2 (June 2022)
3. --
Identification and contact of the 1. RCP: Floor covering
coordinator (s): • Luís Arroja | arroja@ua.pt
• Marisa Almeida | marisa@ctcv.pt
2. RCP: Wall covering
• Luís Arroja | arroja@ua.pt
• Marisa Almeida | marisa@ctcv.pt
Identification and contact of the 1. RCP: Floor covering
authors: • Marisa Almeida | marisa@ctcv.pt
• Luís Arroja | arroja@ua.pt
• Ana Cláudia Dias | acdias@ua.pt
2. RCP: Wall covering
• Marisa Almeida | marisa@ctcv.pt
• Luís Arroja | arroja@ua.pt
DAPHabitat System 4
• Ana Cláudia Dias | acdias@ua.pt
Composition of the Sectorial Panel: 1. RCP: Floor covering
• RMC - Revestimentos de Mármore Compactos, S.A.
• Dominó – Indústrias Cerâmicas, S.A.
• APICER – Associação Portuguesa da Indústria de Cerâmica
• Sonae Indústria, SGPS, S.A.
2. RCP: Wall covering
• RMC - Revestimentos de Mármore Compactos, S.A.
• Dominó – Indústrias Cerâmicas, S.A.
• Sonae Indústria, SGPS, S.A.
• APICER – Associação Portuguesa da Indústria de Cerâmica
Consultation period: 1. 01/08/2013 - 30/11/2013
2. 12/08/2013 - 30/11/2013
Valid until: 1. 01/06/2027
2. 01/06/2027
1.8. Information concerning the product/product class
Identification of the product: Glazed vitrified white body tiles for wall and floor covering
Illustration of the product:
Brief description of the product: Glazed vitrified tiles produced by the PAVIGRÉS CERÂMICAS, S.A group, are used as floor
and wall coverings, indoors and outdoors in residential and public areas. This product is
waterproof and has a high mechanical resistance, being available in the market a panoply
of aesthetic and dimensional options, as much in visual effects as of texture and colours.
In this EPD, the results are provided per unit area (1 m²) of the product for an average
product with a specific weight of 16.41 kg/m². However, the production process (A1-A3) is
the same regardless of the thickness or format of the products. Table 1 presents the
specific weight of the several product thicknesses.
Table 1: Product thicknesses and their weights
Thickness (mm) Weight (Kg/m2)
6 12.9
7.2 15.8
8.3 17.9
Note: Table of average weights per m2 (kg/m2), depending on the thickness of the
product. For more accurate information on each reference’s weights per unit area, please
consult the weights and packaging table on the PAVIGRÉS website.
Main technical characteristics of the
Table 2: Technical characteristics of glazed vitrified tiles products
product:
Designation Average value of tolerances Test standard
Linear dimensions ± 0,3%
Dimensional Orthogonality ± 0,3%
NP EN ISO 10545-2
characteristics Straightness ± 0,3%
Planarity ± 0,3%
DAPHabitat System 5
Thickness ± 3%
Water absorption ≈1,5% NP EN ISO 10545-3
(6mm) ≥ 720 N
Mechanical flexural (7mm) ≥ 1050 N
strength (N)
NP EN ISO 10545-4
(8,3mm) ≥ 1500 N
Rupture modulus
≥ 40 N/mm2
(N/mm2)
Resistance to surface Indicated for each ref NP ISO 10545-7
abrasion
Thermal shock Resistant NP EN ISO 10545-9
resistance
Frost resistance Resistant NP EN ISO 10545-12
Cracking resistance Guaranteed NP EN ISO 10545-11
Resistance to
household cleaning Guaranteed NP EN ISO 10545-13
products and pool
additives
Resistance to
low/high To be confirmed case by case
NP EN ISO 10545-13
concentration acids
and bases
Stain resistance Guaranteed NP EN ISO 10545-14
Below the limit of quantification:
Cadmium and lead < 0,2 mg Pb/l NP EN ISO 10545-15
release < 0,02 mg Cd/l
Anti-slip features To be confirmed case by case According to the
(slipperiness) requested test
Description of the product’s Glazed vitrified tiles in the following applications:
application/use: • Floor covering
• Wall covering
• Indoor covering
• Outdoor covering
• Areas and residential buildings
• Areas and public buildings
• Areas and industrial buildings
Placing on the market / Rules of EN 14411:2012
application in the market / Technical NP EN ISO 10545
rules of the product: DIN 51130
DIN 51097
ENV 12633
BS 7976-2
Quality control:
Under the technical standards of the product
Special delivery conditions:
Not applicable
Components and substances to declare: Not applicable
Where explanatory material may be https://www.pavigres.com/
Quality and environmental standards following ISO 9001:2015 and ISO14001:2015 and
obtained: the provisions described in the relevant regulations.
The product can be found through resellers and professional applicators.
History of the LCA studies:
CTCV, 2019 Project report including the glazed vitrified tiles LCA, to sustain the 2019 EPD
DAPHabitat System 6
1.9. Calculation rules of the LCA
Functional unit: --
Declared unit: 1 m2 of glazed vitrified white body tiles for wall and floor covering
System boundaries: Cradle-to-grave and module D EPD (A1-D)
Criteria for the exclusion: According to point 6.3.5 of NP EN 15804, the exclusion criterion for unitary processes is 1%
of the total energy consumed and 1% of the total mass of the inputs, with special attention
to not exceeding a total of 5% of energy and mass flows excluded in the product stage.
The following processes were not considered in this study, as they may fall within the
exclusion criteria or scope of the standard:
• Environmental loads associated with the construction of industrial infrastructures and the
manufacture of machinery and equipment;
• Environmental loads related to infrastructure (production and maintenance of vehicles
and roads) for transporting pre-products;
• Long-term emissions.
Assumption and limitations For processes over which producers have no influence or specific information, such as the
extraction of raw materials, generic data from the Ecoinvent v3.7 databases were used.
The dataset used to model the production of electricity and natural gas was adapted to the
national reality. The electricity mix was updated for the year 2022 using information from
the National Energy Networks (REN), the Energy Services Regulatory Entity (ERSE) and the
General Directorate of Energy and Geology (DGEG), to consider more recent information
regarding the environmental impacts generated by the electricity network in Portugal. The
natural gas process was modelled according to the information provided by the Energy in
Portugal (2022) report (DGEG), regarding the countries of origin of its import.
The environmental impacts presented in this DAP are a simple average of all PAVIGRES
products manufactured in glazed vitrified tiles in 2022 (since they are only produced in one
industrial unit).
Quality and other characteristics The production data collected corresponds to 2022 and is in accordance with reality. The
generic data used belong to the Ecoinvent v3.7 databases and comply with the quality
about the information used in the criteria (age, geographic and technological coverage, plausibility, etc.) of generic data.
LCA:
Allocation rules: The allocation rules adopted were based on the annual production at the Pavigrés
manufacturing unit.
Software used for the assessment: SimaPro 9.2
Background database used for the Ecoinvent 3.7
LCA:
Comparability of EPD for construction The EPD of construction products and services cannot be comparable if they are not
products produced according to EN 15804 and EN 15948 and according to the comparability
conditions determined by ISO 14025.
1.10. Use of average environmental performance
The glazed vitrified ceramic coverings included in the study are made with the same raw materials and auxiliary
materials, using the same energy resources and technological process, and covering different models with various
formats. The average thickness of the formats included in this EPD is from 6.0 to 8.3 mm, with a mean mass of
16.41 kg/m2.
DAPHabitat System 7
1.11. Technical information for Reference Service Life (RSL)
Parameter Units Results**
Reference Service Life Years Minimum 50
See Table 2
Declared product properties (at the gate) Units as appropriate For more information, contact Pavigrés or
and finishes, etc.
request its technical sheets
Design application parameters (if instructed
For more information, contact Pavigrés or
by the manufacturer), including the Units as appropriate
references to the appropriate practices and request its technical sheets
application codes
For more information, contact Pavigrés or
An assumed quality of work, when installed Units as appropriate
per the manufacturer’s instructions request its technical sheets
Outdoor environment (for outdoor
applications), e.g. weathering, pollutants, Units as appropriate Not Applicable
UV and wind exposure, building orientation,
shading, temperature
Values of relevant characteristics in
Indoor environment (for indoor accordance with Annex H of EN 14411.
applications), e.g. temperature, moisture, Units as appropriate
For more information, contact Pavigrés or
chemical exposure
request technical data sheets.
Values of relevant characteristics in
accordance with Annex H of EN 14411.
Usage conditions, e.g. frequency of use, Units as appropriate
chemical exposure For more information, contact Pavigrés or
request technical data sheets.
Values of relevant characteristics in
accordance with Annex H of EN 14411.
Maintenance, e.g. required frequency, Units as appropriate
mechanical exposure For more information, contact Pavigrés or
request technical data sheets
** expressed by functional unit or declared unit
DAPHabitat System 8
1.12. Flow diagram of input and output of the processes
Figure 1: The life cycle stages of the glazed vitrified tiles products (A1-D).
Production stage, A1-A3
The A1 to A3 stages included the extraction of raw materials, their transport to the factory, and the manufacturing
of the product.
A1 – Extraction and processing of raw materials: this stage includes the extraction and eventual processing of raw
materials.
DAPHabitat System 9
A2 – Transport: The raw materials and auxiliary materials come by tanker truck or by tanker truck, boat and tanker
truck again.
A3 – Production: This stage includes design and development, storage of raw materials, paste preparation, shaping
(by pressing), drying, glazing or decorating, firing and sorting, subsequent treatment (e.g. polishing), packaging and
storage.
Pavigrés Cerâmicas, SA. (at its Pavigrés, Grespor, Cerev and Pavigrés II units) is dedicated to the production of
ceramic tiles (flooring and coverings, in porcelain and non-porcelain stoneware, glazed and unglazed) by pressing
atomized powder, followed by drying and firing. Natural raw materials, synthesized raw materials and additives
are used, the main ones being: clays, feldspars, sands, carbonates and kaolin.
The hard raw materials (such as sands, feldspars, etc.) are subjected to grinding, while the clayey materials
undergo turbo-dilution; subsequently, they are mixed and homogenized (storage and agitation), forming the final
composition of the ceramic body.
The ceramic paste in the form of slip is subsequently atomized (sprayed and dried), forming the ceramic powder
which, after homogenization, is pressed and shaped by pressing. The raw pressed tiles are subjected to a quick
drying cycle to remove residual moisture and, finally, are subjected to the firing process, which will give them all
the final physical and chemical characteristics.
Use stage, B1-B7
B1 - Use or application of the installed product - The environmental impacts generated during the use stage are
very low and, therefore, can be neglected following the EN 17160:2019 standard relating to Product category rules
for ceramic tiles.
B2 - Maintenance - Throughout its useful life, the ceramic coating product must be cleaned regularly, to a greater
or lesser extent, depending on the type of building: residential, commercial, sanitary, etc., where it is installed.
Cleaning agents such as detergents can be added if the surface is dirty or oily. Therefore, the consumption of water
and detergent can be considered.
DAPHabitat System 10
According to the EN 17160:2019 standard regarding Product category rules for ceramic tiles, we have the
“Scenario for maintaining ceramic floor tiles”:
• Residential use: 0.134 ml detergent and 0.1 l of water are used to wash 1 m2 of ceramic floor covering
(tile) once a week.
Washing the product was considered during the useful life of the coating (50 years).
B3 – Repair - Ceramic tiles do not require repair during the use stage; therefore, no impact must be declared at
this stage, per EN 17160:2019 on Product Category Rules for Ceramic Tiles.
B4 – Replacement - Ceramic tiles do not require replacement during the use stage and therefore no impact must
be declared in this replacement stage.
B5 – Rehabilitation - Ceramic tiles do not require rehabilitation during the use stage. Therefore no impact must be
declared at this stage, following EN 17160:2019 regarding Product Category Rules for Ceramic Tiles.
B6 – Energy requirements during the operational stage - Generally, environmental impacts generated during
phase B6 are not applicable and therefore not considered, according to EN 17160:2019 on Product Category Rules
for Ceramic Tiles.
B7 – Water requirements during the operational stage - Generally, environmental impacts generated during
phase B7 are not applicable and therefore neglected, according to EN 17160:2019 regarding Product Category
Rules for Ceramic Tiles.
End of life stage (C1-C4)
C1 – Deconstruction/demolition: According to EN 17160:2019 regarding product category rules for ceramic tiles,
we have the following: “The environmental impacts generated during the C1 phase are very low and therefore can
be neglected.” Therefore, environmental impacts can be ignored.
C2 – Transport to waste processing: According to EN 17160:2019 regarding Product Category Rules for Ceramic
Tiles, we have an average distance of 20 km.
C3 – Waste processing for reuse, recovery and/or recycling: The coating end of life scenarios were based on Table
17 of EN 17160:2019 on Product Category Rules for Ceramic Tiles. Corresponding to:
- 70% recycling;
C4 – Elimination: According to the EN 17160:2019 standard, it was considered 30%.
Potential for reuse, recovery and/or recycling, expressed in net impacts or benefits (D): According to EN
17160:2019 on Product Category Rules for Ceramic Tiles:
DAPHabitat System 11
After the demolition/deconstruction phase, ceramic tiles can be crushed and used in a variety of different
applications:
• concrete aggregates [2];
• when ceramic tiles are crushed, they form recycled ceramic aggregates that can be integrated as a
partial replacement for natural aggregate in hot asphalt mixes;
• recycled ceramic aggregates can be used in the construction of landfills [8];
• recycled ceramic aggregates can be used to construct base sub-layers on secondary roads [8].
It was considered a replacement of 70% of natural aggregates.
DAPHabitat System 12
2. CORE ENVIRONMENTAL IMPACT INDICATORS
2.1. Description of the system boundaries
(✓= included; ND = module not declared)
BENEFITS AND LOADS
CONSTRUCTION
PRODUCT STAGE USE STAGE END OF LIFE STAGE BEYOND THE SYSTEM
PROCESS STAGE
BOUNDARY
la
y lp p u s la ire ta m w a R tro p s n a rT g n iru tc a fu n a M tro p s n a rT s s e c o rp n o ita lla ts n i n o itc
u
e s U e c n a n e tn ia M ria p e R tn e m e c a lp e R tn e m h s ib ru fe R e s u y g re n e la n o ita re p O e s u re ta w la n o ita re p O n o itilo m e d ,s n o itc u rts n eo Dc - tro p s n a rT g n is s ee tc so a Wrp la s o p s iD
itn
e to p g n ilc y c e r ,y re v o c e r ,e es u
-
rts R
n
o
C
A1 A2 A3 A4 A5 B1 B2 B3 B4 B5 B6 B7 C1 C2 C3 C4 D
✓ ✓ ✓ ✓ ✓ ✓ ✓ ✓ ✓ ✓ ✓ ✓ ✓ ✓ ✓ ✓ ✓
Modules A1-A3 include those processes that provide energy and material input for the system (A1), transport up
to the factory gate of the plant (A2), manufacturing processes (A3), and waste processing.
Module A4 includes the transport from the production site to the customer or to the tile’s installation point. Three
scenarios were considered for the transport: 300 km (truck), 1390 km (truck) and 6520 km (ship) according to EN
17160.
Module A5 considers all tile installation steps (like adhesives consumption) and packaging waste processing
(recycling, incineration, disposal). The default values were according to EN 17160. Credits from energy substitution
are declared in module D.
Module B1 considers the use of tiles. No hazardous indoor emissions are expected to occur during the use of
ceramic tiles.
Module B2 includes preventive and regular maintenance activities, such as cleaning, correcting or repairing
damaged or degraded parts. The use of water and wastewater is included in this module.
Modules B3-B4-B5 are related to the tile’s repair, replacement and refurbishment. No repair, replacement or
refurbishment processes are necessary if the tiles are appropriately installed. For this reason, Modules B3-B4-B5
are not considered according to EN17160.
DAPHabitat System 13
Modules B6-B7 consider energy use for operating building integrated technical systems and operational water use
for technical building-related systems (heating systems, cooling, ventilation, lighting, hot water, etc.). No
operational energy or water use are considered. Cleaning water is declared under B2.
Module C1 refers to the demolition and de-construction process of the tiles from the building. According to
EN17160 it is considered negligible.
Module C2 considers the transportation of the discarded tile to a recycling or disposal process. It was considered
20 km.
Module C3 considers every process (collection, crushing process etc.) properly for recycling the tiles (70% following
EN17160).
Module C4 includes all the landfill disposal processes, including pre-treatment and management of the disposal
site (20 km) (30% following EN17160).
Module D includes benefits or burdens to the environment generated by reusable products, recyclable materials,
and/or energy carriers that exit a product system.
2.1.1. Justification for the exemption to declare modules C1, C2, C3, C4 and D
Not applicable.
DAPHabitat System 14
2.2. Core environmental impact indicators
Global Global warming Depletion
Global
warming Global warming potential land use potential of the
warming
potential potential biogenic; and land use stratospheric Acidification
potential total;
fossil; change; ozone layer; potential; AP
GWP-biogenic
GWP-total
GWP-fossil GWP-luluc ODP
Unit kg CO2 eq. kg CO2 eq. kg CO2 eq. kg CO2 eq. kg CFC 11 eq. mol H+ eq.
Modules A1-A3 9.12E+00 9.62E+00 -5.21E-01 1.38E-02 4.51E-07 2.45E-02
Module A4 Scenario A4.1 9.25E-04 7.35E-01 2.22E-04 1.44E-05 1.59E-08 9.25E-04
Scenario A4.2 4.28E-03 3.41E+00 1.03E-03 6.67E-05 7.36E-08 4.28E-03
Scenario A4.3 3.20E-02 1.02E+00 1.56E-04 3.41E-05 1.53E-08 3.20E-02
Module A5 Scenario A5.1 2.57E-03 9.40E-01 3.33E-01 5.37E-04 1.58E-08 2.57E-03
Module B1 Scenario B1.1 0.00E+00 0.00E+00 0.00E+00 0.00E+00 0.00E+00 0.00E+00
Module B2 Scenario B2.1 4.07E-03 5.37E-01 5.14E-03 3.72E-04 4.08E-08 4.07E-03
Module B3 Scenario B3.1 0.00E+00 0.00E+00 0.00E+00 0.00E+00 0.00E+00 0.00E+00
Module B4 Scenario B4.1 0.00E+00 0.00E+00 0.00E+00 0.00E+00 0.00E+00 0.00E+00
Module B5 Scenario B5.1 0.00E+00 0.00E+00 0.00E+00 0.00E+00 0.00E+00 0.00E+00
Module B6 Scenario B6.1 0.00E+00 0.00E+00 0.00E+00 0.00E+00 0.00E+00 0.00E+00
Module B7 Scenario B7.1 0.00E+00 0.00E+00 0.00E+00 0.00E+00 0.00E+00 0.00E+00
Module C1 Scenario C1.1 0.00E+00 0.00E+00 0.00E+00 0.00E+00 0.00E+00 0.00E+00
Module C2 Scenario C2.1 6.16E-05 4.90E-02 1.48E-05 9.60E-07 1.06E-09 6.16E-05
Module C3 Scenario C3.1 7.21E-04 8.94E-02 7.13E-04 4.41E-05 1.48E-09 7.21E-04
Module C4 Scenario C4.1 4.20E-04 5.36E-02 5.17E-05 1.18E-05 9.31E-10 4.20E-04
Module D Scenario D.1 -1.66E-04 -2.08E-02 -1.20E-03 -5.40E-06 -3.54E-10 -1.66E-04
LEGEND:
Product stage
Construction process stage
Use stage
End of life stage
Benefits and loads beyond the system boundary
NOTES1:
Units expressed by functional unit or declared unit.
The life cycle stages (or scenarios) not considered in the study can be eliminated of the table, through the function “eliminate lines” .
1 These annotations should be eliminated for the presentation of the final document
DAPHabitat System 15
Eutrophication Abiotic Abiotic
Eutrophication Formation
p ao qt uen att ii ca l potential Eu ptr oo tp eh nic ta iati lo n potential of pod te ep nle tit aio l fn o r pod te ep nle tit aio l fn o r W dea pte rir
v
( au ts ioe nr)
freshwater; aquatic terrestrial; tropospheric non-fossil fossil potential;
marine; ozone; resources resources
potential
EP- EP-terrestrial WDP
EP-marine POCP ADP-
freshwater minerals&metals ADP-fossil
m3 World eq.
Units kg P eq. kg N eq. mol N eq. Kg COVNM eq. kg Sb eq. MJ, P.C.I
deprived
Modules A1-A3 8.62E-05 5.24E-03 4.81E-02 2.17E-02 1.45E-04 1.42E+02 -2.90E+00
Module A4 Scenario A4.1 5.78E-07 2.29E-04 2.23E-03 1.72E-03 2.53E-08 9.78E+00 8.95E-03
Scenario A4.2 2.68E-06 1.06E-03 1.03E-02 7.97E-03 1.17E-07 4.53E+01 4.15E-02
Scenario A4.3 7.32E-07 8.01E-03 8.87E-02 2.35E-02 1.10E-08 1.25E+01 1.10E-02
Module A5 Scenario A5.1 1.21E-05 6.63E-04 6.91E-03 2.25E-03 4.36E-06 7.52E+00 5.05E-02
Module B1 Scenario B1.1 0.00E+00 0.00E+00 0.00E+00 0.00E+00 0.00E+00 0.00E+00 0.00E+00
Module B2 Scenario B2.1 1.67E-05 4.93E-04 5.40E-03 2.27E-03 2.66E-07 1.84E+01 1.11E+01
Module B3 Scenario B3.1 0.00E+00 0.00E+00 0.00E+00 0.00E+00 0.00E+00 0.00E+00 0.00E+00
Module B4 Scenario B4.1 0.00E+00 0.00E+00 0.00E+00 0.00E+00 0.00E+00 0.00E+00 0.00E+00
Module B5 Scenario B5.1 0.00E+00 0.00E+00 0.00E+00 0.00E+00 0.00E+00 0.00E+00 0.00E+00
Module B6 Scenario B6.1 0.00E+00 0.00E+00 0.00E+00 0.00E+00 0.00E+00 0.00E+00 0.00E+00
Module B7 Scenario B7.1 0.00E+00 0.00E+00 0.00E+00 0.00E+00 0.00E+00 0.00E+00 0.00E+00
Module C1 Scenario C1.1 0.00E+00 0.00E+00 0.00E+00 0.00E+00 0.00E+00 0.00E+00 0.00E+00
Module C2 Scenario C2.1 3.85E-08 1.53E-05 1.49E-04 1.15E-04 1.68E-09 6.52E-01 5.97E-04
Module C3 Scenario C3.1 1.64E-06 3.10E-04 3.38E-03 1.00E-03 3.91E-09 1.33E+00 4.94E-03
Module C4 Scenario C4.1 6.51E-08 1.95E-04 2.11E-03 6.31E-04 2.19E-09 7.09E-01 9.07E-04
Module D Scenario D.1 -1.73E-07 -7.38E-05 -8.06E-04 -2.45E-04 -8.72E-09 -4.05E-01 -6.15E-03
LEGENDA:
Product stage
Construction process stage
Use stage
End of life stage
Benefits and loads beyond the system boundary
NOTES2: P.C.I. – Net calorific value
Units expressed by functional unit or declared unit.
2 These annotations should be eliminated for the presentation of the final document
DAPHabitat System 16
2.3. Additional environmental impact indicators
Potential Potential
Potential
Potential Human Potential Comparative
Comparative
incidence of exposure Comparative Toxic Unit Potential soil
Toxic Unit for
disease due to efficiency Toxic Unit for for humans, quality index
humans, cancer
PM emissions relative to ecosystems not cancer
effects
U235 effects SQP
PM ETP-fw
HTP-c
IRP HTP-nc
Disease
Unit kBq U 235 eq. CTUe CTUh CTUh -
incidence
Modules A1-A3 1.40E-06 1.25E-01 5.46E+01 2.72E-09 6.19E-08 8.82E+01
Module A4 Scenario A4.1 4.43E-08 1.56E-03 4.34E+00 4.56E-11 5.06E-09 1.86E-02
Scenario A4.2 2.05E-07 7.21E-03 2.01E+01 2.11E-10 2.34E-08 8.61E-02
Scenario A4.3 2.43E-08 1.37E-03 6.01E+00 1.52E-10 2.47E-09 1.74E-02
Module A5 Scenario A5.1 6.45E-08 2.06E-02 2.83E+00 2.25E-10 4.83E-09 7.10E+00
Module B1 Scenario B1.1 0.00E+00 0.00E+00 0.00E+00 0.00E+00 0.00E+00 0.00E+00
Module B2 Scenario B2.1 3.80E-08 1.41E-02 1.30E+00 8.65E-10 1.70E-08 8.31E-01
Module B3 Scenario B3.1 0.00E+00 0.00E+00 0.00E+00 0.00E+00 0.00E+00 0.00E+00
Module B4 Scenario B4.1 0.00E+00 0.00E+00 0.00E+00 0.00E+00 0.00E+00 0.00E+00
Module B5 Scenario B5.1 0.00E+00 0.00E+00 0.00E+00 0.00E+00 0.00E+00 0.00E+00
Module B6 Scenario B6.1 0.00E+00 0.00E+00 0.00E+00 0.00E+00 0.00E+00 0.00E+00
Module B7 Scenario B7.1 0.00E+00 0.00E+00 0.00E+00 0.00E+00 0.00E+00 0.00E+00
Module C1 Scenario C1.1 0.00E+00 0.00E+00 0.00E+00 0.00E+00 0.00E+00 0.00E+00
Module C2 Scenario C2.1 2.95E-09 1.04E-04 2.89E-01 3.04E-12 3.37E-10 1.24E-03
Module C3 Scenario C3.1 1.20E-07 3.40E-03 4.89E-01 8.19E-12 2.95E-10 3.95E-01
Module C4 Scenario C4.1 5.52E-08 1.38E-04 3.41E-01 5.22E-12 2.06E-10 2.51E-01
Module D Scenario D.1 -5.04E-09 -3.80E-03 -1.24E-01 -1.13E-11 -7.39E-11 -1.93E+00
LEGEND:
The impact indicator “POTENTIAL HUMAN EXPOSURE EFFICIENCY RELATIVE TO
Product stage U235” focuses mainly on the possible impact of a low dose of ionising radiation
on human health resulting from the nuclear fuel cycle. It does not consider
Construction process stage effects arising from possible nuclear accidents, occupational exposure or the
disposal of radioactive waste in underground facilities. This indicator also does
Use stage
not measure potential ionising radiation from soil, radon and some building
End of life stage materials.
The results of the indicators “POTENTIAL COMPARATIVE TOXIC UNIT FOR
Benefits and loads beyond the system boundary ECOSYSTEMS (ETP-FW)”, “POTENTIAL COMPARATIVE TOXIC UNIT FOR
HUMANS, CANCER EFFECTS”, “POTENTIAL COMPARATIVE TOXIC UNIT FOR
NOTES3: HUMANS, NOT CANCER EFFECTS” and “POTENTIAL SOIL QUALITY INDEX” should
Units expressed by functional unit or declared unit. be used with caution as the uncertainties associated with them are high or
The life cycle stages (or scenarios) not considered in the study can there is little experience with the indicator.
be eliminated of the table, through the function “eliminate lines” .
3 These annotations should be eliminated for the presentation of the final document
DAPHabitat System 17
2.4. Indicators describing resource use
Primary energy
EPR RR TRR EPNR RNR TRNR
Unit MJ, P.C.I. MJ, P.C.I. MJ, P.C.I. MJ, P.C.I. MJ, P.C.I. MJ, P.C.I.
Modules A1-A3 1.73E+01 9.32E-07 1.73E+01 1.56E+02 3.88E-06 1.56E+02
Module A4 Scenario A4.1 1.39E-02 0.00E+00 1.39E-02 1.00E+01 0.00E+00 1.00E+01
Scenario A4.2 6.42E-02 0.00E+00 6.42E-02 4.63E+01 0.00E+00 4.63E+01
Scenario A4.3 1.59E-02 0.00E+00 1.59E-02 1.29E+01 0.00E+00 1.29E+01
Module A5 Scenario A5.1 1.28E+00 2.19E-01 1.50E+00 8.53E+00 0.00E+00 8.53E+00
Module B1 Scenario B1.1 0.00E+00 0.00E+00 0.00E+00 0.00E+00 0.00E+00 0.00E+00
Module B2 Scenario B2.1 4.37E-01 0.00E+00 4.37E-01 2.06E+01 0.00E+00 2.06E+01
Module B3 Scenario B3.1 0.00E+00 0.00E+00 0.00E+00 0.00E+00 0.00E+00 0.00E+00
Module B4 Scenario B4.1 0.00E+00 0.00E+00 0.00E+00 0.00E+00 0.00E+00 0.00E+00
Module B5 Scenario B5.1 0.00E+00 0.00E+00 0.00E+00 0.00E+00 0.00E+00 0.00E+00
Module B6 Scenario B6.1 0.00E+00 0.00E+00 0.00E+00 0.00E+00 0.00E+00 0.00E+00
Module B7 Scenario B7.1 0.00E+00 0.00E+00 0.00E+00 0.00E+00 0.00E+00 0.00E+00
Module C1 Scenario C1.1 0.00E+00 0.00E+00 0.00E+00 0.00E+00 0.00E+00 0.00E+00
Module C2 Scenario C2.1 9.24E-04 0.00E+00 9.24E-04 6.67E-01 0.00E+00 6.67E-01
Module C3 Scenario C3.1 7.10E-02 0.00E+00 7.10E-02 1.40E+00 0.00E+00 1.40E+00
Module C4 Scenario C4.1 1.25E-02 0.00E+00 1.25E-02 7.33E-01 0.00E+00 7.33E-01
Module D Scenario D.1 -1.64E-01 0.00E+00 -1.64E-01 -4.72E-01 0.00E+00 -4.72E-01
LEGEND:
Product stage
Construction process stage
Use stage
End of life stage
Benefits and loads beyond the system boundary
EPR = use of renewable primary energy excluding renewable primary energy resources used as raw materials; RR = use of renewable primary energy resources
used as raw materials; TRR = total use of renewable primary energy resources (EPR + RR); EPNR = use of non-renewable primary energy excluding non-renewable
primary energy resources used as raw materials; RNR = use of non-renewable primary energy resources used as raw materials; TRNR = total use of non-renewable
primary energy resources (EPRN + RNR);
NOTE4: Units expressed by functional units or declared units.
4 These annotations should be eliminated for the presentation of the final document
DAPHabitat System 18
Secondary materials and fuels, and use of water
MS CSR CSNR Net use of fresh water
Unit kg MJ, P.C.I. MJ, P.C.I. m3
Modules A1-A3 5.37E-01 0.00E+00 0.00E+00 -4.85E-02
Module A4 Scenario A4.1 0.00E+00 0.00E+00 0.00E+00 3.06E-03
Scenario A4.2 0.00E+00 0.00E+00 0.00E+00 8.65E-04
Scenario A4.3 0.00E+00 0.00E+00 0.00E+00 1.75E-04
Module A5 Scenario A5.1 0.00E+00 0.00E+00 0.00E+00 1.72E-03
Module B1 Scenario B1.1 0.00E+00 0.00E+00 0.00E+00 0.00E+00
Module B2 Scenario B2.1 0.00E+00 0.00E+00 0.00E+00 2.69E-01
Module B3 Scenario B3.1 0.00E+00 0.00E+00 0.00E+00 0.00E+00
Module B4 Scenario B4.1 0.00E+00 0.00E+00 0.00E+00 0.00E+00
Module B5 Scenario B5.1 0.00E+00 0.00E+00 0.00E+00 0.00E+00
Module B6 Scenario B6.1 0.00E+00 0.00E+00 0.00E+00 0.00E+00
Module B7 Scenario B7.1 0.00E+00 0.00E+00 0.00E+00 0.00E+00
Module C1 Scenario C1.1 0.00E+00 0.00E+00 0.00E+00 0.00E+00
Module C2 Scenario C2.1 0.00E+00 0.00E+00 0.00E+00 1.24E-05
Module C3 Scenario C3.1 0.00E+00 0.00E+00 0.00E+00 3.35E-04
Module C4 Scenario C4.1 0.00E+00 0.00E+00 0.00E+00 4.05E-05
Module D Scenario D.1 0.00E+00 0.00E+00 0.00E+00 -3.98E-03
LEGEND:
Product stage
Construction process stage
Use stage
End of life stage
Benefits and loads beyond the system boundary
MS = use of secondary material; CSR = use of renewable secondary fuels; CSNR = use of non-renewable secondary fuels.
NOTE5: Units expressed by functional units or declared units.
5 These annotations should be eliminated for the presentation of the final document
DAPHabitat System 19
2.5. Other environmental information describing different waste categories
Hazardous waste disposed Non-hazardous waste disposed Radioactive waste disposed
Unit kg kg kg
Modules A1-A3 5.67E-04 1.79E+00 1.00E-04
Module A4 Scenario A4.1 2.50E-05 3.94E-04 6.83E-05
Scenario A4.2 1.16E-04 1.83E-03 3.16E-04
Scenario A4.3 7.14E-06 5.80E-04 8.76E-05
Module A5 Scenario A5.1 2.12E-05 1.52E-01 2.45E-05
Module B1 Scenario B1.1 0.00E+00 0.00E+00 0.00E+00
Module B2 Scenario B2.1 9.78E-06 1.78E-02 1.54E-05
Module B3 Scenario B3.1 0.00E+00 0.00E+00 0.00E+00
Module B4 Scenario B4.1 0.00E+00 0.00E+00 0.00E+00
Module B5 Scenario B5.1 0.00E+00 0.00E+00 0.00E+00
Module B6 Scenario B6.1 0.00E+00 0.00E+00 0.00E+00
Module B7 Scenario B7.1 0.00E+00 0.00E+00 0.00E+00
Module C1 Scenario C1.1 0.00E+00 0.00E+00 0.00E+00
Module C2 Scenario C2.1 4.16E-06 6.57E-05 1.14E-05
Module C3 Scenario C3.1 2.53E-06 2.00E+00 9.41E-06
Module C4 Scenario C4.1 1.80E-06 5.91E+00 5.01E-06
Module D Scenario D.1 -6.56E-07 -5.38E-04 -4.14E-06
LEGENDA:
Product stage
Construction process stage
Use stage
End of life stage
Benefits and loads beyond the system boundary
NOTE6: Units expressed by functional units or declared units.
The characteristics that make waste hazardous are described in the applicable legislation in force, for example, in the European Waste Framework
Directive.
6 These annotations should be eliminated of the presentation of the final document
DAPHabitat System 20
2.6. Environmental information describing output flows
Exported energy
Components for Materials for Materials for energy
re-use recycling recovery
Energy carrier 1
Unit kg kg kg MJ
Modules A1-A3 0.00E+00 5.25E-01 6.41E-03 1.43E+00
Module A4 Scenario A4.1 0.00E+00 0.00E+00 0.00E+00 ND
Scenario A4.2 0.00E+00 0.00E+00 0.00E+00 ND
Scenario A4.3 0.00E+00 0.00E+00 0.00E+00 ND
Module A5 Scenario A5.1 0.00E+00 4.75E-01 8.59E-02 1.38E+01
Module B1 Scenario B1.1 0.00E+00 0.00E+00 0.00E+00 ND
Module B2 Scenario B2.1 0.00E+00 0.00E+00 0.00E+00 ND
Module B3 Scenario B3.1 0.00E+00 0.00E+00 0.00E+00 ND
Module B4 Scenario B4.1 0.00E+00 0.00E+00 0.00E+00 ND
Module B5 Scenario B5.1 0.00E+00 0.00E+00 0.00E+00 ND
Module B6 Scenario B6.1 0.00E+00 0.00E+00 0.00E+00 ND
Module B7 Scenario B7.1 0.00E+00 0.00E+00 0.00E+00 ND
Module C1 Scenario C1.1 0.00E+00 0.00E+00 0.00E+00 ND
Module C2 Scenario C2.1 0.00E+00 0.00E+00 0.00E+00 ND
Module C3 Scenario C3.1 0.00E+00 1.38E+01 0.00E+00 ND
Module C4 Scenario C4.1 0.00E+00 0.00E+00 0.00E+00 ND
Module D Scenario D.1 0.00E+00 0.00E+00 0.00E+00 ND
LEGEND:
Product stage
Construction process stage
Use stage
End of life stage
Benefits and loads beyond the system boundary
ND: Not Declared
DAPHabitat System 21
2.7. Information describing the biogenic carbon content at the factory gate
Biogenic carbon content* Units** Modules A1-A3 (results)
Biogenic carbon content in product Kg C Not applicable (inorganic product)
Biogenic carbon content in accompanying packaging Kg C 1.29E-01
* 1 kg biogenic carbon is equivalent to 44/12 kg of CO2.
** This information can be omitted whenever the content of biogenic carbon in the product, or in the respective packaging, is less than 5% of the
mass of the product, or the respective packaging.
3. SCENARIOS AND ADDITIONAL TECHNICAL INFORMATION7
3.1. A4 Transport to the building site – Construction process stage
The scenarios for A4 transport to the building site were according to EN 17160 regarding Product category rules for
ceramic tiles.
Destination Type of transport Average distance (km)
National – Scenario A4.1 Truck with a capacity of 25 tons 300
Europe – Scenario A4.2 Truck with a capacity of 25 tons 1 390
International (Outside Europe) –
Transoceanic freight ship 6520
Scenario A4.3
3.2. A5 Installation of the product in the building – Construction process stage
The scenario was also according to the options defined in EN17160 and Almeida, 2019, for the installation stage.
The option chosen was 3.3 kg of cementitious adhesive for each m2 of ceramic tile. The ceramic material loss was
considered to be 3%.
Option 3 (medium size tiles) Value Unit of measure
Cementitious adhesive 3.3 kg
7 IF THERE IS NO ADDITIONAL TECHNICAL INFORMATION AND NO SCENARIOS HAVE BEEN CARRIED OUT, ENTRIES SHOULD BE FILLED IN WITH "NOT APPLICABLE”.
DAPHabitat System 22
3.3. B1 Use stage
According to the specific PCR for Product category rules for ceramic tiles - EN 17160, the environmental impacts
generated during the use phase are very low and therefore can be neglected. Ceramic tiles are robust and have a
hard, abrasion-resistant surface.
There are no impacts on the environment during the use stage.
3.4. B2 Maintenance
Ceramic covering products shall be cleaned regularly, depending on the type of building: residential, commercial,
and healthcare. Thus, the consumption of water and cleaning agents has been considered. The values declared in
this stage refer to a period of 50 years. The scenario for maintaining ceramic floor tiles was conservative, according
to EN 17160.
The scenario used for maintaining ceramic floor tiles was for residential use, using 0.134 ml detergent and 0.1 l
water to wash 1 m2 of ceramic floor tiles once a week.
Parameter Value Unit of measure
Water consumption 0.1 l
Detergent consumption 0.134 ml
Floor tile maintenance cycle 2600 Number per RSL
3.5. B3 Repair
In general, the service life of ceramic tiles is the same as the building lifetime. Repair, replacement and
refurbishment are not required for ceramic tiles.
Thus, according to EN 17160, ceramic tiles require no repair during the use phase; therefore, no impact should be
declared during the repair phase.
3.6. B4 Replacement
In general the service life of ceramic tiles is the same as the building lifetime. Repair, replacement and
refurbishment are not required for ceramic tiles.
DAPHabitat System 23
3.7. B5 Rehabilitation
This module is not relevant for ceramic tiles, according to EN 17160.
3.8. B6 Use of energy (operational)
This module is not relevant for ceramic tiles, according to EN 17160.
3.9. B7 Use of water (operational)
This module is not relevant for ceramic tiles, according to EN 17160.
3.10. C1 De-construction, demolition – End of life of the product
C1: Following the PCR developed in EN 17160, this module is irrelevant for ceramic tiles.
3.11. C2 Transport – End of life of the product
C2: The ceramic tile demolition waste is transported by truck from the building site to a container or treatment
plant. An average distance of 20 km is considered, according to the default scenario of EN17160.
3.12. C3 Waste processing for reuse, recovery and/or recycling – End of life of the product
C3 the end-of-life scenario is described in the following table:
Destination Value Unit of measure
Recycling (C3) 70 %
3.13. C4 Disposal – End of life of the product
C4: the end of life scenario is described in the following table:
Destination Value Unit of measure
Landfill (C4) 30 %
3.14. Scenario and technical information for module D
Module D includes credits from materials recycling of tiles and packaging and energy credits from thermal recovery
of the packaging.
According to EN 17160, after the demolition/deconstruction stage, ceramic tiles can be crushed and then used in a
range of different applications:
DAPHabitat System 24
• Aggregates for road construction;
• Concrete aggregates;
• When ceramic tiles are crushed, they form recycled ceramic aggregates, which can be integrated
as a partial substitute for natural aggregate in hot-mix asphalt [8];
• Recycled ceramic aggregates can be used in the construction of landfills [8];
• Recycled ceramic aggregates can be utilized to construct sub-based courses on secondary roads
[8].
In this case, and according to the Environmental Nacional Agency (APA, 2020), in Portugal the valorisation rate of
ceramic materials in construction and demolition waste is approximately 75%.
3.15. Additional information on release of dangerous substances to indoor air, soil, and
water during the use stage
The correct use of the product does not display any danger to water, air or soil. It is inert when used correctly.
The product is classified with A+ (source:Pavigrés self-declaration and CeramUnie guide).
DAPHabitat System 25
4. REFERENCES
✓ Almeida. M. (2019). Desempenho ambiental de produtos no sector cerâmico em Portugal. Tese de
doutoramento. Universidade de Aveiro.
✓ Direção-Geral de Energia e Geologia (DGEG) – Energy in Portugal Report (2019)
✓ Direção-Geral de Energia e Geologia (DGEG) – Monthly Data of Electrical Energy (2019). (em
http://www.dgeg.gov.pt?cr=15125)
✓ Ecoinvent database v3.7 (2019). (www.ecoinvent.org)
✓ EN 15804:2012+A2:2019 Sustentabilidade das obras de construção. Declarações ambientais de produtos.
Regras fundamentais para a categoria de produto dos produtos de construção.
✓ EN 15942:2011 Sustentabilidade na construção – declaração ambiental de produto – Comunicação no
formato empresa-empresa
✓ EN 17160:2019 – “Product category rules for ceramic tiles”.
✓ Entidade Reguladora dos Serviços Energéticos (ERSE) – Produção em Regime Especial Renovável (PRE)
(2019 e 2020) (em http://www.erse.pt/pt/desempenhoambiental/prodregesp/2019/Paginas/2019.aspx)
✓ Instruções Gerais do Sistema DAPHabitat, Versão 1.0, Março de 2013 (em www.daphabitat.pt);
✓ NP ISO 14025:2009 Rótulos e declarações ambientais – Declarações ambientais Tipo III – Princípios e
procedimentos;
✓ RCP – modelo base para produtos e serviços de construção. Sistema DAPHabitat. Versão 2.2, Janeiro de
2016 (em www.daphabitat.pt);
✓ Redes Energéticas Nacionais (REN) – Information Centre – Monthly Statistics (2022). (em
http://www.centrodeinformacao.ren.pt/PT/InformacaoExploracao/Paginas/EstatisticaMensal.aspx)
✓ PCR – basic module for construction products and services. DAPHabitat System. Version 2.3, agosto de
2023 (em www.daphabitat.pt);
✓ Regras para a Categoria de Produto (RCP) – Revestimento de Paredes. RCP002:2014. Sistema
DAPHabitat. Versão 1.2, Junho 2022 (em www.daphabitat.pt);
✓ Regras para a Categoria de Produto (RCP) – Revestimento de Pavimento. RCP001:2014. Sistema
DAPHabitat. Versão 1.2, Junho 2022 (em www.daphabitat.pt).
DAPHabitat System 26
