Environmental Product
Declaration
as per ISO 14025 and EN 15804
Owner of the declaration: SIA ARBO Windows
Publisher: Kiwa-Ecobility Experts
Program operator: Kiwa-Ecobility Experts
Registration number: EPD-ArboWindows-242-EN
Issue date: 02-03-2023
Valid to: 01-03-2028
76/105 PANEL DOORS
___________
PANEL DOOR – WOOD
1. General information
SIA ARBO Windows 76/105 Group panel doors
Programme operator Owner of the declaration
Kiwa-Ecobility Experts SIA ARBO Windows
Kiwa GmbH Kustes dambis 32
Voltastr. 5 Ventspils, LV-3601
13355 Berlin Latvia
Germany
Declaration number Declared product / declared unit
EPD-ArboWindows-242-EN 1 m2 of product
This declaration is based on the Product Scope
Category Rules
Group 76/105 Panel Door wood has a thermal
EN 17213:2020 Windows and doors – transmittance of 0,99 W/(m2*K). The
Environmental Product Declarations – Product dimensions (height x width) are made
category rules for windows and pedestrian according to the customer's requirements.
doorsets (PCR B) The calculation is based on the assumption
that LCA results are scalable for the desired
Issue date
door dimension. The product is manufactured
02.03.2023 in Ventspils, Latvia, and marketed
internationally.
Valid to
Kiwa-Ecobility Experts shall not be liable with
01.03.2028 respect to manufacturer information, life
cycle assessment data and evidence.
Verification
The standard EN 15804+A2:2019 serves as the
core PCR
Independent verification of the declaration
and data according to ISO 14025:2006
☐internally ☒externally
Frank Huppertz
(Head of Kiwa-Ecobility Experts)
Prof. Dr. Frank Heimbecher Natalia Chebaeva
(Chairman of the independent expert committee – (External verifier – Ecomatters)
Ecobility Experts)
Page | 2 SIA ARBO Windows – Group 76/105 Panel Doors Wood
2. Product
2.1 Product description
This EPD covers the 76/105 Group Panel doors wood. Dimensions (height x width) are adapted
according to customer's requirements. The results are an average of the whole group.
76/105 Group Panel doors includes the following products:
• 76/105 profile panel doors – wood.
Figure 1: 76/105 wooden panel door Figure 2: 76/105 wooden panel door
2.2 Application
The products are used as enclosures for openings in facades of buildings. The indented uses are in
domestic and commercial locations.
UN CPC code: 42120
2.3 Placing on the market / Application rules
The harmonized standard for windows and pedestrian doorsets is EN 14351-1. The CE mark is applied
to the finished products. According to the Construction Products Regulation CPR (EU) No. 305/2011,
the essential properties of products are declared in the CE marking and Declaration of Performance.
The factory production control of SIA ARBO Windows conforms to requirements of above mentioned
standard according to system 3. Factory production control ensures the quality of the products.
SIA ARBO Windows meets requirements of the following additional certifications:
• P-MARK;
• NDVK (Norwegian Door-And Window Control);
• FSC®;
• Management system certifications: ISO 9001:2015, ISO 14001:2015 and ISO 50001:2018.
Market: Norway, Sweden, Denmark, United Kingdom, Finland and elsewhere. Waste scenarios are
calculated for Norwegian market.
Page | 3 SIA ARBO Windows – Group 76/105 Panel Doors Wood
2.4 Technical data
For the description of the declared performances Regulation (EU) No. 305/2011 is used. The
harmonized standard for windows and pedestrian doorsets is EN 14351-1.
Technical Data – 76/105 Wooden Panel doors
Characteristic Value Unit
Type 76/105 wooden panel door -
Glass type - -
Total Weight* 25,07 kg
Thickness x width 105 x 72 mm
Glass surface* - m2
Heat permeability, window (U -value) (EN 10077) 0,99 W/(m2*K)
w
Safety equipment n.a. -
Sound insulation n.a. db
Air permeability (EN 1026) Class 4 -
Water tightness (EN12208) 9A -
Resistance to wind load, test pressure Class 4 -
(EN 12210)
Resistance to wind load, frame deflection (EN 12210) Class C -
Dangerous substances None
Note: * Reference size 1m2
The indicated technical parameters may change if changes are made in the configuration of the glass
package and in other cases of application of technical solutions without changing the product materials
and technology.
2.5 Base materials / Ancillary
Characteristic Value Unit
Type 76/105 wooden panel door -
Wood (pine) 20,00 kg
Steel 2,40 kg
Aluminium 0,67 kg
Plastics (diverse materials)* 1,10 kg
Paint, impregnant, primer 0,90 -
Note: * mixture of TPE, PVC, PP
2.6 Information on biogenic carbon content
Name Value Unit
Product 9,09 kg C
Packaging 0,00 kg C
Note: 1 kg biogenic carbon is equivalent to 44/12 kg CO2.
2.7 Manufacturing
The manufacturing contains the following processes:
• Extraction and delivery of raw materials;
• Cutting and profiling;
• Impregnation;
• Assembly of frame;
Page | 4 SIA ARBO Windows – Group 76/105 Panel Doors Wood
• Priming and painting of frame;
• Assembly of complete product;
• Packing and delivery.
Figure 3: Overview of the production route of a door (A1-A3, C1-C4, D)
2.8 Packaging
The finished product is placed and fixed on pallets in a vertical position. The corners of the product are
covered by cardboard. All products on the pallet are covered by packing film. Wrapping the pallet
with a wrapping film protects the products from short-term exposure to moisture, transport dust and
other adverse effects during transportation. The transportation does not cause any losses as products
are secured properly.
2.9 Production waste
The data on generated production waste is recorded as accurately as possible. Thus, the generated
production waste is allocated per declared unit. There is no production waste for metal, because steel
and aluminium hardware is delivered of the size as in the drawings (no cutting is made). Other
materials such as plastics (diverse material) and aluminium profiles are cut to the required size.
Page | 5 SIA ARBO Windows – Group 76/105 Panel Doors Wood
3. LCA: Calculation rules
3.1 Declared unit
In accordance with PCR B (EN 17213), one square meter was chosen as the declared unit for a door
representing the 76/105 Group Panel Doors. Further information for describing the declared unit can
be found in the table below.
Declared units – Group 76/105 Panel Doors Wood
Description Value Unit
Type 76/105 wooden panel door -
Declared unit 1 m2
Frame: material type Pine -
Frame: mass 20,00 kg
Seal: material type TPE / Silicone -
Seal: mass 0,812 / 0,150 kg
Hardware and profile: material type Steel / aluminium -
Hardware and profile: mass 2,40 / 0,67 kg
Total mass 25,07 kg
Conversion factor to 1 kg 0,040 m2/kg
3.2 System boundary
This Life cycle assessment is made for EPD type "Cradle to gate with modules C1-C4 and module D":
The Environmental Product Declaration analyses the Production stage (A1-A3), the End-of-Life stage
(C1-C4) and the Benefits and loads beyond the system boundary (D).
In a typical panel door manufacturing process, the individual components such as framing materials,
hardware (hinges, locks, handles etc.), impregnant, sealant, primers, paints and other ancillary
materials are delivered to the manufacturing site. The processes that are performed at the
manufacturing site are: cutting and profiling, impregnation, assembly of frame, treatment and coating,
assembly of complete product, packing and delivery. All inputs including raw materials, primary
products, energy and auxiliary materials as well as the accumulated waste, are considered in the
assessment.
Production stage
A1: This stage considers the extraction and processing of raw materials as well as energy consumption.
All installed raw materials of the products were analysed, and the masses were determined.
A2: The raw materials are transported to the manufacturing plant. In this case, the model includes
road/ maritime transportation of each raw material. Supplier information regarding the transport
distances and vehicle type were provided by SIA ARBO Windows or chosen from relevant market
profiles.
A3: This stage includes the manufacture of products and packaging. It also considers the energy
consumption and waste generated at the manufacturing site. The national electricity mix of Latvia was
taken into account.
Page | 6 SIA ARBO Windows – Group 76/105 Panel Doors Wood
Assembly stage
A4: Transportation of assembly stage is not declared.
A5: Installation process is not declared. The packaging is not modelled in C-D modules as it is discarded
in module A5 which is not declared.
Use stage
B1 to B7: The use of the final product is not within the manufacturer's sphere of influence. Therefore,
modules B1-7 have not been considered.
End of life stage
C1: Demolition concerns the removal of the door, whereby no environmental impact is assumed (e.g.
emissions to air, water or soil). No information was found in the life cycle databases consulted for the
dismantling operations of windows/ doors, nor was there a bibliography regarding the inputs or
residues generated during these operations. Then dismantling is assumed at the site (so transport in
C1 would be 0 km). Therefore there is no contribution on impact categories of this module. The
resulting waste materials and quantities are included in the respective modules.
C2: Transport module concerns transportation to waste processing. All of end-of-life product is
assumed to be sent to the closest facilities (C2).
Transport to waste processing (C2)
Name Vehicle type Distance
Truck* Lorry (Truck), unspecified (default) | market group Landfill:100 km; Incineration: 150
for (GLO) km (energy recovery on site 0);
Recycling: 50 km; Re-Use: 0 km
Note: * For all transports, the environmental profile of a non-specific truck transport was used (conservative
assumption): The vehicle operates with diesel, and it provides a fleet average that includes different lorry classes
as well as EURO classes. This transport used an average load factor, including empty return trips.
C3 and C4: At the end-of-life is based on the assumption that all material components after their
service life are disassembled to a specific waste flow (e.g. wood, metal, plastic and glass). The individual
parts are assigned to the material-specific disposal route – waste processing (C3) for reuse, recovery
and/or recycling) or landfill (C4).
End of life (C1-C4)
Name Value Unit
Collected separately waste type 25,07 kg
Collected as mixed construction waste 0,00 kg
Re-use 0,00 kg
Recycle 2,92 kg
Energy recovery 20,20 kg
Landfilling 1,25 kg
3.3 Estimates and assumptions
All installed raw materials of the product were analysed, and the masses were determined following
the allocation and cut-off requirements. Production-specific energy consumption were measured and
provided by SIA ARBO Windows.
Page | 7 SIA ARBO Windows – Group 76/105 Panel Doors Wood
Since the production process is quite similar for all of the products produced at the manufacturing site,
the energy consumption, ancillary materials and production waste is allocated according to the annual
production of the standard sized elements and then declared per square meter of the product. The
total annual production data is recorded to a high standard of accuracy and precision.
The production waste of wood, paint and other mixed production waste is collected separately. Wood
waste is thermally recovered at the site. As the product is marketed internationally, no country-specific
waste scenario can be considered. Therefore, the waste scenario of PCR B (EN 17213 Appendix B.3)
was adopted. Removing the door does not result in any emissions to air or soil, so the value for module
C1 is assumed to be zero.
3.4 Cut-off criteria
The study does not exclude any modules or processes which are stated mandatory in the EN 15804
and applicable PCR. The study does not exclude any hazardous materials or substances included in the
Candidate List of Substances of Very High Concern (SVHCs) for authorization with concentrations
higher than 0.1% weight by weight. All material flows that contribute to more than 1% of the total
mass, energy or environmental impact of the system have been considered in the LCA. It can be
assumed that the neglected processes in total contributed less than 5% to the considered impact
categories.
The product stage includes materials, energy and waste flows only related to production processes
(e.g. energy and water use related to company management and sales activities are excluded where
technically possible; production, manufacture, and construction of manufacturing capital goods and
infrastructure, other processes which are not directly related to the production of windows and doors).
3.5 Background Data
The Life Cycle Assessment was modelled with the R<THiNK software from NIBE. The background data
is taken from Ecoinvent version 3.6 (2019) “Allocation, cut-off” database. Geographical reference
space of the background data is Europe or Global. Almost all consistent datasets contained in the
Ecoinvent database are documented and can be viewed in the online Ecoinvent documentation. The
reference year to collect all input data is 2021. The geographical reference area is Europe or Global
and can be seen in the system description boundary table.
3.6 Data quality
In the operating data survey all relevant process-specific data has been collected. The data relating to
the manufacturing phase of the doors was determined by SIA ARBO Windows.
Secondary data was taken from the Ecoinvent 3.6 (2019) database. The database is regularly checked
and thus complies with the requirements of ISO 14040/44 (background data is not older than 10 years).
The background data meets the requirements of EN 15804.
The general rule was followed that specific data from specific production processes or average data
derived from specific processes must be given priority when calculating an EPD or Life Cycle
Assessment. Data for processes that the manufacturer cannot influence or choose, were backed up
with generic data.
Page | 8 SIA ARBO Windows – Group 76/105 Panel Doors Wood
3.7 Period Under review
All process-specific data was collected for the manufacturing year 2021. The quantities of raw and
ancillary materials as well as energy consumption have been recorded and averaged over the entire
operating year 2021.
3.8 Allocation
There are no co-products in the raw material supply and manufacturing phase, therefore no allocation
methods were used at this stage (for co-products). Appropriation or attribution of inputs and outputs,
e.g. auxiliary materials, energy (utilities), waste have been done on the basis of production volumes in
2021 (reference year), taking into account an area of a standard sized doors (as per PCR B EN 17213),
e.g. door size 1,23 m x 2,18 m (area of a door 2,68 m2). The Life Cycle Assessment was modelled with
the R<THiNK software from NIBE. The background data is taken from Ecoinvent version 3.6 (2019)
Allocation, cut-off library. Almost all consistent datasets contained in the Ecoinvent database is
documented and can be viewed in the online Ecoinvent documentation. Allocation principles in the
background are in compliance with the foreground. Specific information on allocations within the
background data can be found in the Ecoinvent database version 3.6 (2019) document.
3.9 Calculation methods
For life cycle assessment, the calculation methods described in ISO 14040 have been applied. The
evaluation is based on the phases in the system boundaries.
3.10 Mix of electricity and CO -Certificates
2
The electricity mix (medium voltage) was chosen, using the country-specific market dataset (Latvia)
from the background database. Reference year of the dataset 2019, reference year of the electricity
mix is at least 2012. The Ecoinvent profile used for the gridmix includes the imported energy and
excludes the exported energy.
3.11 Comparability
EPD of construction products may not be comparable if they do not comply with the requirements of
EN 15804. Basically, a comparison or an evaluation of EPD data is only possible if all the data sets to be
compared were created according to EN 15804 and the building context, respectively the product-
specific characteristics of performance, are considered.
3.12 Reference Service Life (RSL)
According to the standard EN 17213 a reference service life of 30 years is assumed without IGU
replacement. This is on the basis that the installation, maintenance and servicing of the product follows
the relevant instructions of the manufacturer which are submitted to every customer and also
available on the web page of SIA ARBO Windows. It should be noted that the Use stage with modules
B1-B7 is not declared.
Page | 9 SIA ARBO Windows – Group 76/105 Panel Doors Wood
4. System boundary description and LCA results
This Life cycle assessment is made for EPD type “cradle to gate with modules C1-C4 and module D”.
The Environmental Product Declaration analyses the Production stage (A1-A3), the end-of-life stage
(C1-C4) and the Benefits and loads beyond the system boundary (D).
System boundary description
Description of the system boundary
Benefits and
Construction loads beyond
Production stage Use stage End of life stage
process stage the system
boundaries
y lp p u s la ir e t a m w a R t r o p s n a r T g n ir u t c a fu n a M u n a m m o r f t r o p s n a r T-e s u fo e c a lp o t r e r u t c a
f
n on io t cit ua rl tl sa nts on C-is s e c o r p e s U e c n a n e tn ia M r ia p e R tn e m e c a lp e R n e m h s ib r u fe Rt y g r e n e la n o it a r ee ps Ou e s u r e t a w la n o it a r e p O / n o it c u r ts n eo Dc -n o itilo m e d t r o p s n a r T g n is s e c o r p e ts a W la s o p s iD y r e v eo s uc ee RR -- gla ni it ln c ye ct o e Rp -
A1 A2 A3 A4 A5 B1 B2 B3 B4 B5 B6 B7 C1 C2 C3 C4 D
X X X MND MND MND MND MND MND MND MND MND X X X X X
Geography
EU, EU, LV, EU,
MND MND MND MND MND MND MND MND MND EU EU EU EU, GLO
GLO GLO EU NO
X=Module declared | MND=Module not declared
All major materials, production energy use and waste are included for phases A1, A2, A3, C1, C2, C3
and C4. Use stage B1-B7 is not relevant for this type of product and is not declared.
The following tables show the results of the impact assessment indicators, resource use, waste and
other output streams. The results presented refer to the declared average product.
Disclaimer on ADP-e, ADP-f, WDP, ETP-fw, HTP-c, HTP-nc, SQP: The results of these environmental
impact indicators must be used with caution, as the uncertainties in these results are high or as there
is limited experience with the indicator.
Disclaimer on IR: This impact category mainly addresses the potential effect of low dose ionizing
radiation on human health in the nuclear fuel cycle. It does not consider effects due to possible nuclear
accidents and occupational exposures, nor does it consider radioactive waste disposal in underground
facilities. Potential ionizing radiation from soil, radon, and some building materials is also not measured
by this indicator.
Page | 10 SIA ARBO Windows – Group 76/105 Panel Doors Wood
Results of the LCA for 76/105 Group Panel Door Wooden
Results of the LCA: Environmental impact of 1 m2 panel door
Parameter Unit A1 A2 A3 C1 C2 C3 C4 D
Core environmental impact indicators (EN 15804)
ADP-f MJ 4,47E+02 4,12E+01 1,82E+02 0,00E+00 6,93E+00 5,97E+00 3,19E-01 -2,92E+02
ADP-mm kg Sb-eqv. 1,48E-03 6,37E-05 6,06E-05 0,00E+00 1,16E-05 1,08E-05 3,80E-08 2,62E-03
AP mol H+ eqv. 2,05E-01 1,77E-02 8,73E-02 0,00E+00 2,67E-03 8,90E-03 1,18E-04 -8,30E-02
EP-fw kg P eqv. 1,53E-03 4,23E-05 1,86E-04 0,00E+00 4,64E-06 2,10E-05 3,83E-07 -3,51E-04
EP-m kg N eqv. 3,72E-02 5,43E-03 1,77E-02 0,00E+00 9,39E-04 3,50E-03 6,82E-05 -1,25E-02
EP-T mol N eqv. 4,06E-01 6,04E-02 2,11E-01 0,00E+00 1,04E-02 4,00E-02 4,13E-04 -1,46E-01
GWP-b kg CO2 eqv. -3,30E+01 2,67E-03 4,68E+00 0,00E+00 2,12E-04 3,22E+01 1,77E+00 -3,26E-01
GWP-f kg CO2 eqv. 3,30E+01 2,83E+00 1,20E+01 0,00E+00 4,60E-01 3,56E+00 2,27E-02 -1,95E+01
GWP-luluc kg CO2 eqv. 1,90E-01 1,56E-03 1,81E-02 0,00E+00 1,68E-04 4,20E-04 7,75E-06 -1,16E-01
GWP-total kg CO2 eqv. 2,15E-01 2,83E+00 1,67E+01 0,00E+00 4,60E-01 3,58E+01 1,80E+00 -1,99E+01
ODP kg CFC 11 eqv. 2,88E-06 5,77E-07 1,91E-06 0,00E+00 1,01E-07 1,28E-07 4,08E-09 -2,73E-06
POCP kg NMVOC eqv. 1,33E-01 1,83E-02 5,86E-02 0,00E+00 2,96E-03 1,05E-02 1,46E-04 -5,07E-02
WDP m3 world eqv. 9,35E+00 1,76E-01 2,21E+00 0,00E+00 2,48E-02 2,22E-01 1,39E-02 -7,61E-01
Additional environmental impact indicators (EN 15804)
ETP-fw CTUe 8,88E+02 4,43E+01 2,15E+02 0,00E+00 6,18E+00 4,84E+01 2,10E+01 -1,72E+02
HTP-c CTUh 7,69E-08 3,18E-09 1,35E-08 0,00E+00 2,01E-10 7,76E-08 8,38E-12 -1,99E-08
HTP-nc CTUh 1,11E-06 5,07E-08 1,47E-07 0,00E+00 6,76E-09 3,95E-08 3,23E-10 9,87E-08
IR kBq U235 eqv. 1,37E+00 1,75E-01 8,28E-01 0,00E+00 2,90E-02 2,29E-02 1,24E-03 -9,78E-01
PM disease incidence 3,29E-06 2,63E-07 2,03E-06 0,00E+00 4,14E-08 7,76E-08 2,13E-09 -7,86E-07
SQP Pt 5,36E+03 2,48E+01 7,30E+02 0,00E+00 6,01E+00 4,18E+00 7,26E-01 -8,87E+01
ADP-e=Depletion of abiotic resources-elements | ADP-f=Depletion of abiotic resources-fossil fuels | AP=Acidification of soil and water | EP-fw =Eutrophication, freshwater | EP-m=Eutrophication marine | EP-
T=Eutrophication, terrestrial | GWP-b=Global warming potential – Biogenic | GWP-f=Global warming potential – Fossil | GWP-luluc=Global warming potential – Land use and land use change |GWP-total=Global warming
potential |ODP=Ozone layer depletion |POCP=Photochemical oxidants creation | WDP=Water use | ETP-fw=Ecotoxicity, freshwater | HTP-c=Human toxicity, cancer | HTP-nc=Human toxicity, non-cancer | IR=Ionising
radiation, human health | PM=Particulate Matter | SQP=Land use
Page | 11 SIA ARBO Windows – Group 76/105 Panel Doors Wood
Results of the LCA: Resource use and environmental information of 1 m2 panel door
Parameter Unit A1 A2 A3 C1 C2 C3 C4 D
PERE MJ 4,84E+02 8,30E-01 1,28E+02 0,00E+00 8,68E-02 5,71E-01 9,91E-03 -6,99E+01
PERM MJ 2,80E+02 0,00E+00 2,24E+01 0,00E+00 0,00E+00 0,00E+00 0,00E+00 0,00E+00
PERT MJ 7,64E+02 8,30E-01 1,50E+02 0,00E+00 8,68E-02 5,71E-01 9,91E-03 -6,99E+01
PENRE MJ 4,35E+02 4,37E+01 1,94E+02 0,00E+00 7,36E+00 6,37E+00 3,38E-01 -3,17E+02
PENRM MJ 4,04E+01 0,00E+00 1,70E+00 0,00E+00 0,00E+00 0,00E+00 0,00E+00 0,00E+00
PENRT MJ 4,76E+02 4,37E+01 1,96E+02 0,00E+00 7,36E+00 6,37E+00 3,38E-01 -3,17E+02
SM kg 1,18E+00 0,00E+00 0,00E+00 0,00E+00 0,00E+00 0,00E+00 0,00E+00 0,00E+00
RSF MJ 0,00E+00 0,00E+00 0,00E+00 0,00E+00 0,00E+00 0,00E+00 0,00E+00 0,00E+00
NRSF MJ 0,00E+00 0,00E+00 0,00E+00 0,00E+00 0,00E+00 0,00E+00 0,00E+00 0,00E+00
FW m3 3,26E-01 6,39E-03 7,17E-02 0,00E+00 8,44E-04 1,48E-02 3,36E-04 -2,65E-01
HWD kg 4,26E-03 5,23E-04 2,10E-04 0,00E+00 1,76E-05 4,22E-03 2,89E-07 4,87E-03
NHWD kg 7,70E+00 1,67E+00 1,31E+00 0,00E+00 4,40E-01 2,91E-01 1,25E+00 -1,81E+00
RWD kg 1,45E-03 2,64E-04 8,07E-04 0,00E+00 4,55E-05 2,38E-05 1,88E-06 -9,62E-04
CRU kg 0,00E+00 0,00E+00 0,00E+00 0,00E+00 0,00E+00 0,00E+00 0,00E+00 0,00E+00
MFR kg 0,00E+00 0,00E+00 0,00E+00 0,00E+00 0,00E+00 2,92E+00 0,00E+00 0,00E+00
MER kg 0,00E+00 0,00E+00 0,00E+00 0,00E+00 0,00E+00 0,00E+00 0,00E+00 0,00E+00
EE MJ 0,00E+00 0,00E+00 -1,10E+01 0,00E+00 0,00E+00 0,00E+00 0,00E+00 -1,51E+02
EET MJ 0,00E+00 0,00E+00 -6,94E+00 0,00E+00 0,00E+00 0,00E+00 0,00E+00 -9,53E+01
EEE MJ 0,00E+00 0,00E+00 -4,03E+00 0,00E+00 0,00E+00 0,00E+00 0,00E+00 -5,54E+01
PERE=renewable primary energy ex. Raw materials | PERM=renewable primary energy used as raw materials | PERT=renewable primary energy total | PENRE=non-renewable primary energy ex. Raw materials |
PENRM=non-renewable primary energy used as raw materials | PENRT=non-renewable primary energy total | SM=use of secondary material | RSF=use of renewable secondary fuels | NRSF=use of non-renewable secondary
fuels | FW=use of net fresh water | HWD=hazardous waste disposed | NHWD=non-hazardous waste disposed | RWD=radioactive waste disposed | CRU=Components for re-use | MFR=Materials for recycling |
MER=Materials for energy recovery | EE=Exported energy | EET=Exported Energy Thermic | EEE=Exported Energy Electric
Page | 12 SIA ARBO Windows – Group 76/105 Panel Doors Wood
5. LCA: Interpretation
The following figure shows the influence of the different life stages for the 76/105 Group wooden
panel door. As shown in the Figure 4, the most of the environmental impact is attributed to the raw
material processing phase (A1), followed by the transportation of raw materials (A2) and the
production (A3). Potential credits come mainly from the material recovery of aluminium and steel.
Group 76/105 wooden panel doors
100%
50%
0%
-50%
-100%
A1 A2 A3 C1 C2 C3 C4 D
Figure 4: Influence of the modules A1 – A3, C1 – C4 and D on the analysed impact categories for
76/105 Group Panel Door
Overall, the quality of the data can be considered as good overall. The primary data collection has been
done thoroughly. Data quality was calculated using the Data Quality level and criteria according to the
PEF approach (Annex E.2 of EN15804+A2). The DQRs range from 1,67 to 2,67 for the most abundant
inputs in terms of mass.
Page | 13 SIA ARBO Windows – Group 76/105 Panel Doors Wood
6. Additional information: Norwegian requirements
Greenhouse gas emissions from the use of electricity mix in the manufacturing phase
Data source Amount Unit
Ecoinvent 3.6 (year 2019) 0,526 CO2-eqv/kWh
Dangerous substances disclaimer
The product contains no substances given by the REACH Candidate list or the Norwegian
☐
priority list
The product contains substances given by the REACH Candidate list or the Norwegian priority
☒
list that are less than 0,1 % by weight.
The product contain dangerous substances, more then 0,1% by weight, given by the REACH
☐
Candidate List or the Norwegian Priority list, see table.
The product contains no substances given by the REACH Candidate list or the Norwegian
☐ priority list. The product is classified as hazardous waste (Avfallsforskiften, Annex III), see
table.
Indoor environment
The EPD does not give information on release of dangerous substances to indoor air because the
horizontal standards on measurement of release of regulated dangerous substances from construction
products using harmonised test methods according to the provisions of the respective technical
committees for European product standards are not available.
The product contains no dangerous substances on the REACH Candidate list or the Norwegian priority
list, and a water-based release agent is used. Based on this it is assumed that the product has a
negligible impact on the indoor environment.
Soil and water
The EPD does not give information on release of dangerous substances to soil and water because the
horizontal standards on measurement of release of regulated dangerous substances from construction
products using harmonised test methods according to the provisions of the respective technical
committees for European product standards are not available.
Carbon footprint
Carbon footprint has not been worked out for the product.
Page | 14 SIA ARBO Windows – Group 76/105 Panel Doors Wood
7. References
CML-IA, 2013: Characterisation factors developed by Institute of Environmental Sciences (CML):
University Leiden (NL) – http://www.cml.leiden.edu/software/data-cmlia.html
Ecoinvent Database Version 3.6 (2019)
European Commission Joint Research Centre Institute for Prospective Technological Studies (JCR),
Seville, 2014: End-of-waste criteria for waste plastic for conversion
NIBE, 2022: R<THiNK Online-EPD-Tool
Norwegian EPD foundation, Oslo, 2021: NPCR Part A Construction products and services, Version 2.0
Norwegian EPD foundation, Oslo, 2021: NPCR 014 Part B for Windows and doors (references to EN
15804+A2)
Kiwa-Ecobility Experts, Berlin, 2022: PCR A – General Program Category Rules for Construction
Products from the EPD programme of Kiwa-Ecobility Experts; Version 2.1
REACH Regulation (EC) No 1907/2006 of the European Parliament and of the Council on the
Registration, Evaluation, Authorisation and Restriction of Chemicals (REACH)
https://echa.europa.eu/candidate-list-table
Stichting Bouwkwaliteit (SBK), Rijswijk, 2019: Assessment Method – Environmental Performance
Construction and Civil Engineering Works (GWW), , Version "3.0 January 2019" incl. amendments July
2019, Jan 2020
Stichting National Environmental Database (NMD), Rijswijk 2022: Environmental Performance
Assessment Method for Construction Works, Version 1.1.
Stichting National Environmental Database (NMD), Rijswijk, 2019: verification protocol - inclusion data
in the Dutch environmental database
United Nations, New York, 2015 - Central Product Classification (CPC) Version 2.1
Standards
EN 15804:2014 (+A1), Sustainability of construction works – Environmental Product Declarations –
Core rules for the product category of construction products
EN 15804:2020 (+A2), Sustainability of construction works – Environmental product declarations -
Core rules for ,the product category of construction products
EN 16449:2014, Wood and wood-based products – Calculation of the biogenic carbon content of wood
and conversion to carbon dioxide
EN 17213:2020, Windows and doors – Environmental Product Declarations – Product category rules
for windows and pedestrian doorsets
ISO 14025:2006, Environmental labels and declarations – Type III environmental declarations –
Principles and procedures
ISO 14040:2006, Environmental management – Life cycle assessment – Principles and framework
ISO 14044:2006, Environmental management – Life cycle assessment – Requirements and guidelines
ISO 21930:2007, Sustainability in building construction – Environmental declaration of building
products
Page | 15 SIA ARBO Windows – Group 76/105 Panel Doors Wood
Publisher Mail DE.Ecobility.Experts@kiwa.com
Kiwa - Ecobility Experts https://www.kiwa.com/de/de/ub
Kiwa GmbH Web er-kiwa/ecobility-experts/
Voltastr.5, 13355 Berlin
Germany
Programme operator Mail DE.Ecobility.Experts@kiwa.com
Kiwa - Ecobility Experts https://www.kiwa.com/de/de/ub
Kiwa GmbH Web er-kiwa/ecobility-experts/
Voltastr.5, 13355 Berlin
Germany
Author of the Life Cycle Tel. +371 67 607 900
Assessment Mail jekaterina.krastina@kiwa.com
Inspecta Latvia AS Web https://www.kiwa.com/lv
Skanstes iela 54a
Riga, LV-1013
Latvia
Owner of the declaration Tel. +371 67 116 138
SIA ARBO Windows Mail info@arbowindows.lv
Kustes dambis 32 Web https://www.arbowindows.lv/
Ventspils, LV-3601
Latvia
Kiwa-Ecobility Experts -
established member of
Page | 16 SIA ARBO Windows – Group 76/105 Panel Doors Wood
