ENVIRONMENTAL PRODUCT DECLARATION
as per ISO 14025 and EN 15804+A2
Owner of the Declaration ZinCo GmbH
Programme holder Institut Bauen und Umwelt e.V. (IBU)
Publisher Institut Bauen und Umwelt e.V. (IBU)
Declaration number EPD-ZIC-20200082-CCA1-EN
Issue date 31.07.2020
Valid to 30.07.2025
“Heather with Lavender” Green Roof System
ZinCo GmbH
www.ibu-epd.com | https://epd-online.com
Umwelt Produktdeklaration Name des Herstellers – Name des Produkts
General Information
ZinCo GmbH “Heather with Lavender” Green Roof
System
Programme holder Owner of the declaration
IBU – Institut Bauen und Umwelt e.V. ZinCo GmbH
Panoramastr. 1 Lise-Meitner-Straße 2
10178 Berlin 72622 Nürtingen
Germany Germany
Declaration number Declared product / declared unit
EPD-ZIC-20200082-CCA1-EN 1 m² “Heather with Lavender” Green Roof System
This declaration is based on the product Scope:
category rules: This declaration covers the products of ZinCo GmbH,
green roof systems, 12.2019 which is based in Nürtingen. The system components
(PCR checked and approved by the SVR) are mainly produced in Germany. The “Heather with
Lavender” system, which involves simple intensive
roof greening, was selected as a representative
Issue date
system. Information on further system variants can be
31.07.2020
obtained from the manufacturer on request. The
planting of the green roof system does not form a part
Valid to of this declaration.
30.07.2025
The owner of the declaration shall be liable for the
underlying information and evidence; the IBU shall not
be liable with respect to manufacturer information, life
cycle assessment data and evidences.
The EPD was created according to the specifications
of EN 15804+A2. In the following, the standard will be
simplified as EN 15804.
Verification
The standard EN 15804 serves as the core PCR
Independent verification of the declaration and data
according to ISO 14025:2010
Dipl. Ing. Hans Peters internally x externally
(chairman of Institut Bauen und Umwelt e.V.)
Dr. Alexander Röder Matthias Schulz
(Managing Director Institut Bauen und Umwelt e.V.)) (Independent verifier appointed by SVR)
Product
Product description/Product definition Substrate of at least 100 mm in height. It consists
A green roof type “Heather with Lavender” serves to mainly of crushed mineral aggregates and selected
offer a permanent habitat on flat and slightly sloping organic components.
roofs for a certain kind of vegetation, to store water, to The system substrate layer is finally greened by
discharge excess water and to protect the underlying sowing, planting or applying pre-grown vegetation
roof construction. mats; the vegetation itself does not form part of this
The system consists of four or five layers depending EPD.
on whether the roof to be planted is protected against
root penetration or not (see the graphic 1). In exceptional cases of not root resistant
In the case of standard root resistant waterproofing, waterproofing, the waterproofing is first covered with
the Protection Mat SSM 45 is first laid to protect the the Root Barrier WSF 40 or the Root Barrier WSB 100-
waterproofing against mechanical damage and to store PO, depending on the roof situation and/or planting,
rainwater. The mat is covered with 40 mm high before the Protection Mat SSM 45 is laid.The Root
Floradrain® FD 40 drainage and water storage Barriers are not part of this declaration.
elements, equipped on the upper side with recesses
and channels on the lower side. These elements are in
turn covered with the Filter Sheet SF to permanently
guarantee the drainage function.
The Filter Sheet is followed by a layer of System
2 Environmental Product Declaration ZinCo GmbH – Green Roof System
Key Graphic 1: height 100 – 150 mm)
Protection Mat SSM 45 protection Residual
effectiveness in accordance with ≥ 25 thickness
EN ISO 13428 in %
Floradrain® FD 40 compressive
strength in accordance with EN ≥ 115 kPa
ISO 25619-2
Floradrain® FD 40 drainage
capacity in accordance with EN
1.282 l/(m*s)
ISO 12958 at i = 0.02 (rigid/rigid;
20 kPA; bottom side)
Filter Sheet SF penetration force
1100 N
in accordance with EN ISO 12236
System Substrate water storage
approx. 50 Vol.-%
capacity
System Substrate salt content
< 2.5 g/l
(KCl in water extract)
1.0 Roof construction with root resistant waterproofing System Substrate pH (CaCl2) 6,5-8 -
1.1 Protection Mat SSM 45 Fire resistance class for growing
A2 - s1,d0 -
1.2 Floradrain® FD 40 media (EN 13501-1)
1.3 Filter Sheet SF System sound absorption (EN
1.4 System Substrate, at least 100 mm thick ISO 10140-1, EN ISO 10140-2) npd dB
1.5 Vegetation
Product according to CPR with ETA Delivery status
EU regulation no. 305/2011 (CPR) applies for putting Protection Mat SSM 45 is supplied in 100 m² rolls,
the product on the market in the European Floradrain® FD 40 drainage and water storage
Union/European Free Trade Association elements in 2 m² panels and the Filter Sheet SF in 100
EU/EFTA (with the exception of Switzerland). The m² or 200 m² rolls.
product requires a Declaration of Performance taking System Substrate is supplied either as 24 m³ loose by
into account European Technical Assessment ETA- the truck or in Big Bags containing 1 m³.
13/0668 entitled “Kits for Green Roofs” dated 12th
June 2018 and CE labelling. Base materials/Ancillary materials
The respective national regulations apply to use.
The “Heather with Lavender” green roof system
consists of the following components:
Application 97.4 mass % System Substrate
(consisting of approximately 40 % mineral recycling
The “Heather with Lavender” green roof system is granulate, approximately 40 % volcanic loose bulk
applied above the usually root resistant waterproofing materials, approximately 10 % substrate compost, 9 %
on sufficiently stable flat or slightly sloping roofs in sand and approximately 1 % peat)
accordance with the sequence of components 0.1 mass % Filter Sheet SF
described in "Product description/Product definition”. (consisting of 100 % polypropylene (PP))
Roofs greened with this system provide ecological, 2.0 mass % Floradrain® FD 40
urban development and constructional benefits such (consisting of 100 % recycling polyolefin (70 % HDPE,
as the creation of new living space for flora and fauna, 30 % PP))
buffering of areas for microclimate improvement, areas 0.5 mass % Protection Mat SSM 45
for water retention or urban gardening. (consisting of 70 % polyester (PES) and 30 %
polypropylene (PP))
Technical Data
No ancillary materials are required to build the
Amongst others, the requirements of European “Heather with Lavender” green roof system.
Technical Assessment ETA-13/0668 entitled “Kits for
Green Roofs” of 12th June 2018 apply for the “Heather This product contains substances listed in the
with Lavender” green roof system. The performance candidate list (date: 16.01.2020) exceeding 0.1
characteristics which this assessment requires are percentage by mass: no.
shown in the following table:
This product contains other CMR substances in
Constructional data categories 1A or 1B which are not on the candidate
list, exceeding 0.1 percentage by mass: no.
Name Value Unit
System height ≥ 140 mm Biocide products were added to this construction
System weight saturated ≥ 163 kg/m2 product or it has been treated with biocide products
Dry system weight ≥ 103 kg/m² (this then concerns a treated product as defined by the
Maximum system water retention (EU) Ordinance on Biocide Products No. 528/2012):
≥ 60 l/m²
capacity no.
Run-off coefficient Cs of the
system according to the FLL No verification was available for the System Substrate.
0.4 -
Green Roof Guidelines (Roof However, no negative consequences have become
slope up to 5°; System Substrate known in thirty years of use.
3 Environmental Product Declaration ZinCo GmbH – Green Roof System
Reference service life
Professionally fitted Green Roofs last for the life of the
building if cared for and maintained appropriately; ≥ 50
years are possible.
LCA: Calculation rules
Declared Unit Module A5: Installation of Substrate (by vacuum with
The declared unit is one square meter of installed Diesel consumption) and treatment of installation
green roof system without root protection and losses. Treatment of packaging.
vegetation layer. Module B1: Manufacturing of a representative amount
of fertilizer (10 grams of nitrogen per year). Emissions
are not declared since vegetation is not under study.
Name Value Unit Module C1: Deconstruction of the system. Substrate
Grammage (dry) 102.7035 kg/m2 layer is assumed to be vacuumed off the roof (Diesel
Conversion factor to 1 kg (kg/m²) 102.7035 - consumption). All other system components are
Declared unit 1 m2 deconstructed manually (no loads).
Module C2: Transport to EoL treatment (50km
standard distance; may be adapted on building level).
Module C3: Thermal treatment of plastics (European
System boundary Scenario).
Cradle to gate with options, modules C1-C4 and D. Module C4: Disposal of inert and biodegradable waste
(European Scenario).
Description of the system boundaries Module D: Benefits & loads beyond the system
Module A1: Manufacturing processes of system boundaries.
components incl. packaging and treatment of
manufacturing losses from suppliers.Module A2: Comparability
Transport to ZinCo Warehouse. Basically, a comparison or an evaluation of EPD data
Module A3: no loads or benefit is only possible if all the data sets to be compared
Module A4: Transport to building site (100 km standard were created according to EN 15804 and the building
distance, needs to be adapted on building level if context, respectively the product-specific
relevant). characteristics of performance, are taken into account.
The GaBi background database Service Pack 40 has
been used to calculate the EPD results.
LCA: Scenarios and additional technical information
End of life (C1-C4)
Transport to the building site (A4)
Name Value Unit
Name Value Unit Average transport distance to
50 km
Litres of fuel 0.134 l/100km waste treatment facility
Transport distance 100 km Collected separately waste type 102.8 kg
Capacity utilisation (including Energy recovery 2.813 kg
61 - 90 %
empty runs) Landfilling 100 kg
Gross density of products
856.67 kg/m3
transported
Installation into the building (A5) Information on biogenic Carbon
Name Value Unit
Material loss 0.082 kg Biogenic carbon content in packaging (wooden
Diesel consumption 0,15 l/m² pallets): 0,054 kg
Biogenic carbon content in substrate layer (compost):
1,491 kg
Use or application of the installed product (B1)
Name Value Unit
Average fertilizer use per year 0,556 kg/a
Reference service life
Name Value Unit
Life Span (according to BBSR) 40 a
4 Environmental Product Declaration ZinCo GmbH – Green Roof System
LCA: Results
Disclaimer:
EP-freshwater: This indicator has been calculated as “kg P eq” as required in the characterization model
(EUTREND model, Struijs et al., 2009b, as implemented in ReCiPe;
http://eplca.jrc.ec.europa.eu/LCDN/developerEF.xhtml)
DESCRIPTION OF THE SYSTEM BOUNDARY (X = INCLUDED IN LCA; ND = MODULE OR INDICATOR NOT
DECLARED; MNR = MODULE NOT RELEVANT)
BENEFITS AND
CONSTRUCTI LOADS
PRODUCT STAGE ON PROCESS USE STAGE END OF LIFE STAGE BEYOND THE
STAGE SYSTEM
BOUNDARIES
5 Environmental Product Declaration ZinCo GmbH – Green Roof System
lairetam
waR
ylppus tropsnarT
gnirutcafunaM
eht
morf
tropsnarT
etis
eht
ot
etag
ylbmessA esU
ecnanetniaM
riapeR
tnemecalpeR tnemhsibrufeR
ygrene
lanoitarepO esu
retaw
lanoitarepO esu
noitcurtsnoc-eD
noitilomed tropsnarT
gnissecorp
etsaW
lasopsiD -esueR -yrevoceR -gnilcyceR laitnetop
A1 A2 A3 A4 A5 B1 B2 B3 B4 B5 B6 B7 C1 C2 C3 C4 D
X X X X X X ND MNR MNR MNR ND ND X X X X X
RESULTS OF THE LCA - ENVIRONMENTAL IMPACT according to EN 15804+A2: 1 m² "Heather with
Lavender" Green Roof System
Core Indicator Unit A1-A3 A4 A5 B1 C1 C2 C3 C4 D
GWP-total [kg CO2-Eq.] -2.67E+0 4.76E-1 6.94E-1 9.94E-2 5.12E-2 2.38E-1 6.85E+0 1.15E+1 -3.66E-1
GWP-fossil [kg CO2-Eq.] 2.64E+0 4.74E-1 3.92E-1 9.65E-2 7.26E-2 2.37E-1 6.85E+0 2.17E+0 -3.66E-1
GWP-biogenic [kg CO2-Eq.] -5.32E+0 1.90E-4 3.00E-1 2.82E-3 -2.36E-2 9.54E-5 -3.16E-4 9.31E+0 -9.54E-4
GWP-luluc [kg CO2-Eq.] 6.43E-3 1.99E-3 2.24E-3 7.05E-5 2.23E-3 9.93E-4 2.30E-4 4.53E-3 -3.29E-4
ODP [kg CFC11-Eq.] 3.37E-14 1.16E-16 2.36E-16 6.16E-16 1.31E-16 5.82E-17 1.91E-15 6.81E-15 -4.94E-15
AP [mol H+-Eq.] 5.97E-3 3.94E-4 3.72E-4 6.94E-4 2.87E-4 1.97E-4 8.97E-4 1.31E-2 -5.90E-4
EP-freshwater [kg PO4-Eq.] 8.15E-6 1.03E-6 1.18E-6 2.26E-6 1.16E-6 5.17E-7 3.22E-7 4.58E-4 -6.06E-7
EP-marine [kg N-Eq.] 2.43E-3 1.13E-4 7.42E-5 8.21E-5 4.94E-5 5.65E-5 2.41E-4 6.55E-3 -1.45E-4
EP-terrestrial [mol N-Eq.] 2.68E-2 1.39E-3 1.09E-3 8.94E-4 7.01E-4 6.99E-4 4.01E-3 3.83E-2 -1.54E-3
POCP [kg NMVOC-Eq.] 6.39E-3 3.16E-4 2.65E-4 2.58E-4 1.95E-4 1.58E-4 6.90E-4 1.33E-2 -4.10E-4
ADPE [kg Sb-Eq.] 5.24E-7 3.94E-8 4.59E-8 1.91E-7 4.43E-8 1.97E-8 2.82E-8 1.75E-7 -7.23E-8
ADPF [MJ] 4.74E+1 6.30E+0 7.24E+0 2.04E+0 7.08E+0 3.15E+0 2.56E+0 2.91E+1 -6.26E+0
[m³ world-Eq
WDP 1.44E-1 2.04E-3 6.74E-2 3.17E-3 2.30E-3 1.02E-3 7.09E-1 1.71E-1 -4.91E-2
deprived]
GWP = Global warming potential; ODP = Depletion potential of the stratospheric ozone layer; AP = Acidification potential of land and water; EP =
Caption Eutrophication potential; POCP = Formation potential of tropospheric ozone photochemical oxidants; ADPE = Abiotic depletion potential for non-
fossil resources; ADPF = Abiotic depletion potential for fossil resources; WDP = Water use
RESULTS OF THE LCA - RESOURCE USE according to EN 15804+A2: 1 m² "Heather with Lavender"
Green Roof System
Indicator Unit A1-A3 A4 A5 B1 C1 C2 C3 C4 D
PERE [MJ] 1.27E+1 3.66E-1 3.68E+0 1.50E-1 4.12E-1 1.83E-1 5.22E-1 3.12E+0 -1.76E+0
PERM [MJ] 3.24E+0 0.00E+0 -3.24E+0 0.00E+0 0.00E+0 0.00E+0 0.00E+0 0.00E+0 0.00E+0
PERT [MJ] 1.59E+1 3.66E-1 4.44E-1 1.50E-1 4.12E-1 1.83E-1 5.22E-1 3.12E+0 -1.76E+0
PENRE [MJ] 3.20E+1 6.30E+0 8.75E+0 2.04E+0 7.08E+0 3.15E+0 6.96E+0 3.75E+1 -6.26E+0
PENRM [MJ] 1.43E+1 0.00E+0 -1.50E+0 0.00E+0 0.00E+0 0.00E+0 -4.40E+0 -8.40E+0 0.00E+0
PENRT [MJ] 4.63E+1 6.30E+0 7.25E+0 2.04E+0 7.08E+0 3.15E+0 2.56E+0 2.91E+1 -6.26E+0
SM [kg] 5.28E+1 0.00E+0 0.00E+0 0.00E+0 0.00E+0 0.00E+0 0.00E+0 0.00E+0 0.00E+0
RSF [MJ] 0.00E+0 0.00E+0 0.00E+0 0.00E+0 0.00E+0 0.00E+0 0.00E+0 0.00E+0 0.00E+0
NRSF [MJ] 0.00E+0 0.00E+0 0.00E+0 0.00E+0 0.00E+0 0.00E+0 0.00E+0 0.00E+0 0.00E+0
FW [m³] 6.94E-3 3.28E-4 1.91E-3 6.34E-4 3.69E-4 1.65E-4 1.68E-2 5.51E-3 -2.03E-3
PERE = Use of renewable primary energy excluding renewable primary energy resources used as raw materials; PERM = Use of
renewable primary energy resources used as raw materials; PERT = Total use of renewable primary energy resources; PENRE = Use of
non-renewable primary energy excluding non-renewable primary energy resources used as raw materials; PENRM = Use of non-
Caption
renewable primary energy resources used as raw materials; PENRT = Total use of non-renewable primary energy resources; SM = Use
of secondary material; RSF = Use of renewable secondary fuels; NRSF = Use of non-renewable secondary fuels; FW = Use of net fresh
water
RESULTS OF THE LCA – OUTPUT FLOWS AND WASTE CATEGORIES according to EN 15804+A2:
1 m² "Heather with Lavender" Green Roof System
Indicator Unit A1-A3 A4 A5 B1 C1 C2 C3 C4 D
HWD [kg] 4.51E-7 2.36E-7 2.65E-7 1.66E-9 2.65E-7 1.18E-7 8.58E-9 3.12E-7 -2.52E-9
NHWD [kg] 2.10E-1 1.11E-3 2.31E-2 2.15E-1 1.24E-3 5.53E-4 6.27E-1 9.83E+1 -3.32E-3
RWD [kg] 1.18E-3 6.64E-6 1.55E-5 2.45E-5 7.46E-6 3.31E-6 1.06E-4 3.39E-4 -6.01E-4
CRU [kg] 0.00E+0 0.00E+0 0.00E+0 0.00E+0 0.00E+0 0.00E+0 0.00E+0 0.00E+0 0.00E+0
MFR [kg] 0.00E+0 0.00E+0 0.00E+0 0.00E+0 0.00E+0 0.00E+0 0.00E+0 0.00E+0 0.00E+0
MER [kg] 0.00E+0 0.00E+0 0.00E+0 0.00E+0 0.00E+0 0.00E+0 0.00E+0 0.00E+0 0.00E+0
EEE [MJ] 0.00E+0 0.00E+0 1.16E+0 0.00E+0 0.00E+0 0.00E+0 1.51E+1 2.71E+0 0.00E+0
EET [MJ] 0.00E+0 0.00E+0 2.08E+0 0.00E+0 0.00E+0 0.00E+0 2.72E+1 0.00E+0 0.00E+0
HWD = Hazardous waste disposed; NHWD = Non-hazardous waste disposed; RWD = Radioactive waste disposed; CRU = Components
Caption for re-use; MFR = Materials for recycling; MER = Materials for energy recovery; EEE = Exported electrical energy; EEE = Exported
thermal energy
RESULTS OF THE LCA – additional impact categories according to EN 15804+A2-optional:
1 m² "Heather with Lavender" Green Roof System
Indicator Unit A1-A3 A4 A5 B1 C1 C2 C3 C4 D
[Disease
PM ND ND ND ND ND ND ND ND ND
Incidence]
[kBq U235-
IR ND ND ND ND ND ND ND ND ND
Eq.]
ETP-fw [CTUe] ND ND ND ND ND ND ND ND ND
HTP-c [CTUh] ND ND ND ND ND ND ND ND ND
HTP-nc [CTUh] ND ND ND ND ND ND ND ND ND
SQP [-] ND ND ND ND ND ND ND ND ND
PM = Potential incidence of disease due to PM emissions; IR = Potential Human exposure efficiency relative to U235; ETP-fw = Potential
Caption comparative Toxic Unit for ecosystems; HTP-c = Potential comparative Toxic Unit for humans; HTP-nc = Potential comparative Toxic
Unit for humans; SQP = Potential soil quality index
References
DIN EN ISO 13428 EN ISO 14025:2011, Environmental labels and
DIN EN ISO 13428:2005-05, Geosynthetics - declarations - Type III environmental declarations -
Determination of the protection efficiency of a Principles and procedures
geosynthetic against impact damage
ISO 25619-2
ISO 25619-2:2008, Geosynthetics - Determination of
EN 13501-1 compression behaviour - Part 2: Determination of
EN 13501-1:2010, Fire classification of construction short-term compression behaviour
products and building elements - Part 1: Classification
using data from reaction to fire tests IBU 2016, PCR Part A
Product Category Rules for Construction Products
EN 13948 from the range of Environmental Product Declarations
EN 13948:2008, Flexible sheets for waterproofing - of Institut Bauen und Umwelt e.V.(IBU), Part A:
Bitumen, plastic and rubber sheets for roof Calculation Rules for the Life Cycle Assessment and
waterproofing - Determination of resistance to root Requirements of the Background Report. 03/2016,
penetration www.bau-umwelt.com
EN 15804 IBU 2019, PCR Part B
EN 15804:2012-04+A1 2013, Sustainability of PCR-Part B: requirements on the EPD for Green Roof
construction works - Environmental product Systems, Institut Bauen und Umwelt e.V. (IBU);
declarations - Core rules for the product category of 12/2019
construction products
GaBi
EN 15804 GaBi 9 software-system and databases, LBP,
EN 15804:2019-04+A2 (in print), Sustainability of University of Stuttgart and thinkstep, Leinfelden-
construction works - Environmental product Echterdingen, 2019 (http://documentation.gabi-
declarations - Core rules for the product category of software.com/)
construction products
ETA-13/0668
EN ISO 10140-1 European Technical Assessment ETA-13/0668:2018-
EN ISO 10140-1:2016, Acoustics - Laboratory 06-12: “Kits for Green Roofs”
measurement of sound insulation of building
elements - Part 1: Application rules for specific FLL Green Roof Guidelines
products “Guidelines for the Planning, Construction and
Maintenance of Green Roofs” (2018 edition)
EN ISO 10140-2
EN ISO 10140-2:2010, Acoustics - Laboratory REACH
measurement of sound insulation of building REACH EU chemicals directive (EC 1907/2006)
elements - Part 2: Measurement of airborne sound
insulation Regulation (EU) no. 305/2011
Regulation (EU) no. 305/2011 of the European
ISO 12236 Parliament and of the Council - Council Directive
EN ISO 12236:2006, Geosynthetics - Static puncture 89/106/EEC
test (CBR test)
ZinCo System Data Sheet
ISO 12958 “Heather with Lavender with Floradrain® FD 40"
EN ISO 12958:2010, Geotextiles and geotextile-related
products - Determination of water flow capacity in their ZinCo Installation Instructions
plane "System Build-up "Heather with Lavender" with
Floradrain® FD 40"
ISO 14025
ZinCo Product Data Sheets
6 Environmental Product Declaration ZinCo GmbH – Green Roof System
"Root Barrier WSB 100-PO"; "Protection Mat SSM 45";
"Floradrain® FD 40"; "Filter Sheet SF"; "System
Substrate Heather with Lavender"
7 Environmental Product Declaration ZinCo GmbH – Green Roof System
Publisher
Institut Bauen und Umwelt e.V. Tel +49 (0)30 3087748- 0
Panoramastr. 1 Fax +49 (0)30 3087748- 29
10178 Berlin Mail info@ibu-epd.com
Germany Web www.ibu-epd.com
Programme holder
Institut Bauen und Umwelt e.V. Tel +49 (0)30 - 3087748- 0
Panoramastr 1 Fax +49 (0)30 – 3087748 - 29
10178 Berlin Mail info@ibu-epd.com
Germany Web www.ibu-epd.com
Author of the Life Cycle
Assessment Tel +49 711 341817-0
Sphera Solutions GmbH Fax +49 711 341817-25
Hauptstraße 111- 113 Mail info@sphera.com
70771 Leinfelden-Echterdingen Web http://www.sphera.com
Germany
Owner of the Declaration
ZinCo GmbH Tel 07022/6003-0
Lise-Meitner-Strasse 2 Fax 07022/6003-100
72622 Nürtingen Mail info@zinco-greenroof.com
Germany Web www.zinco-greenroof.com
