ENVIRONMENTAL-PRODUCT DECLARATION
as per ISO 14025 and EN 15804+A2
Owner of the Declaration Hilti Aktiengesellschaft
Publisher Institut Bauen und Umwelt e.V. (IBU)
Programme holder Institut Bauen und Umwelt e.V. (IBU)
Declaration number EPD-HIL-20220307-IBA1-EN
Issue date 27/01/2023
Valid to 26/01/2028
HIT-FP 700-R
Hilti AG
www.ibu-epd.com | https://epd-online.com
1. General Information
Hilti AG HIT-FP 700-R
Programme holder Owner of the declaration
IBU – Institut Bauen und Umwelt e.V. Hilti Aktiengesellschaft
Hegelplatz 1 Feldkircher Strasse 100
10117 Berlin 9494 Schaan
Germany Liechtenstein
Declaration number Declared product / declared unit
EPD-HIL-20220307-IBA1-EN The declared product is a HILTI injectable mortar HIT-FP 700-R. The
declared unit is one kilogram of injectable mortar product in the mixing
ratio of the two components necessary for processing. The packaging is
also included in the calculation. The declared unit is stated in [kg].
This declaration is based on the product category rules: Scope:
Reaction resin products, 01/08/2021 This document refers to the injectable mortar HIT-FP 700-R with its
(PCR checked and approved by the SVR) packaging. For the compilation of the life cycle assessment, specific data
were collected from the factory in Kaufering, Germany, of the HILTI AG.
Since the production of this product has only just started in 2022, no
Issue date annual average consumption can be used. The input and output flows
used in this calculation were therefore measured directly by the
27/01/2023
manufacturer for this production process for a comparable product.
The owner of the declaration shall be liable for the underlying information
and evidence; the IBU shall not be liable with respect to manufacturer
Valid to
information, life cycle assessment data and evidences.
26/01/2028
The EPD was created according to the specifications of EN 15804+A2. In
the following, the standard will be simplified as EN 15804 bezeichnet.
Verification
The standard EN 15804 serves as the core PCR
Independent verification of the declaration and data according to ISO
14025:2011
internally X externally
Dipl.-Ing Hans Peters
(chairman of Institut Bauen und Umwelt e.V.)
Dr. Alexander Röder Matthias Klingler,
(Managing Director Institut Bauen und Umwelt e.V.) (Independent verifier)
1 Environmental-Product Declaration - Hilti AG - HIT-FP 700-R
2. Product
Hollow Drill bits and
2.1 Product description/Product definition vacuum cleaners that drill and clean the hole in one step for a
The declared product of HIT-FP virtually dust-free installation. The use of Hilti HDE 500-22
700-R is a two component system. dispenser with the Volume Calculator
The cementitious component (component A) comprises a app leads to no under or over-fill, reducing underfilling-related
reactive compound based on cement and water as well as risks and
inhibitors, viscosity modifying minimizing mortar wastage.
agents and a biocide. The activator component (component B)
comprises of an alkaline 2.3 Technical Data
activator, water, organic acids, viscosity modifying agents and The technical specifications of the products within the scope of
mineral the EPD shall be listed, including the reference to the test
fillers. methods/test standards for each specification.
Mixing the two components A and B in the static mixer initiates
the curing For products with CE marking, the technical specifications must
(hardening) reaction of the cementitious component. During the be specified in accordance with information in the declaration of
curing phase, a mechanical performance. The properties relevant to the product should be
interlock is formed between the inorganic binder and the specified in the table below. If no information is given for
mineral fillers. properties, an explanation must be given in the background
The system formed during the curing process results in an report to the EPD as to why the property is not relevant to the
inorganic microstructure product.
with a hydrate phase assemblage creating the desired design
properties (high Constructional data
fire resistance, required bond strength, creep stability) and
Name Value Unit
particular
long-term stability. Density acc. to EN ISO 1183-3 (standard 2270 kg/m3
The pre-mixed components and the two-component injection climate; after 7 days)
technology exclude dust formation and ensure a proper water- Compressive strength on the basis of DIN
cement ratio during the application of EN 196-1 (storage acc. to DIN EN 196-1; 47 N/mm2
the mortar. after 7 days)
Composite foils are used for the two component foil Tensile shear strength acc. to DIN EN not
N/mm2
pack of HIT-FP 700-R. This kind of packaging serves the 14293 assessed
following purposes:
not
waste volume reduction, easy storage and transport, and less Tensile bond strength acc. to DIN EN 14293 N/mm2
assessed
packaging material.
HIT-FP 700-R is the Hilti
high performance injectable mortar with approvals for rebar HIT-FP 700 R displays the following characteristics:
connections. For the placing of the
product on the market in the European Union European Free
Trade Association
EU/EFTA (with the exception of Switzerland) Regulation (EU) Performance data of the
No. 305/2011 product in accordance with the declaration of performance with
(CPR) applies. The product needs a declaration of performance respect to its essential
taking into characteristics according to
consideration the following European Technical Approval
ETA-21/0624
ETA-21/0624
and the CE
marking. For the application and use the respective national
provisions apply.
2.2 Application Shelf
Hilti HIT-FP 700-R life of 12 months:
serves for safely securing post-installed rebar connections in
cracked and
uncracked concrete C12/15 to C50/60.
Substrate temperature during
Hilti HIT-FP 700-R is a component of the Hilti SAFEset concept. installation 5° to 40°C (internal method).
Hilti SAFEset
is an approved system which makes anchor installation an
easier, safer and
faster process. It significantly improves the robustness of Working time:
fastening and ≥
dramatically reduces the possibility of error during installation. 5 … 10 50 min
As part of >
SAFEset HIT-FP 700-R can be installed with approved Hilti 10 … 15 40 min
2 Environmental-Product Declaration - Hilti AG - HIT-FP 700-R
> All raw materials are sourced from Europe. The transport is
15 … 20 35 min exclusively by truck. Chemical mortars are usually two-
> component systems consisting of a binder and a hardener.
20 … 30 20 min
> The production of chemical mortars consists of a mixing
30 … 40 15 min process and a filling process of the respective single
40 12 min components (binder and hardener/activator) and their
subsequent union to a two-component system (container). Here
as well process control technology is used to weigh and mix
solid and liquid compounds according to specification. In the
next step both well-mixed components run through an
automized filling
line in which each of the processed masses is filled into a
tubular foil bag. Finally the single components are united in one
container. The two-pack foil bags are packed into cardboard
boxes and then finally shipped.
The manufacturing plant of HIT-FP 700-R, Hilti GmbH
Curing time: Industriegesellschaft für Befestigungstechnik, Hiltistr. 6, 86916
≥ Kaufering, Germany, is certified according to ISO 9001. The
5 … 10 50 days guideline defines international standards for quality and
> process management.
10 … 15 28 days
> 2.7 Environment and health during manufacturing
15 … 20 18 days The manufacturing plant of HIT-FP 700-R, Hilti GmbH
> Industriegesellschaft für Befestigungstechnik, Hiltistr. 6, 86916
20 … 30 10 days Kaufering, Germany, is certified according to ISO 14001 which
> defines international standards for sustainable environmental
30 … 40 7 days management. The production site is also certified in
40 4 days accordance with ISO 50001 Energy Management Systems.
2.4 Delivery status 2.8 Product processing/Installation
The product Hilti HIT-FP The product is delivered with Instructions for Use explaining the
700 R is available in foil packages with a total of 490 ml basic steps for installation:
injectable mortar in 1) For safe handling the precautionary measures described in
the corresponding mixing ratio. the Safety Data Sheet (SDS) (e.g. hand and eye protection)
must be adhered to
2.5 Base materials/Ancillary materials 2) Insert the cartridge into the black cassette
Hilti HIT-FP 700-R is supplied in the form of a dual component 3) Screw on the mixing nozzle
film-wrapped pack comprising a cement-based component and 4) Put the cassette into the dispenser system
a limestone-based component at a volume ratio of 3:1. The 5) Discard the first trigger pulls
mixing ratio of cementitious and activator components is 6) Fill 2/3 of the borehole with mortar
automatically set during the injection process. Product curing 7) Set the fixing element
commences directly after the components are mixed. After mixing the components and squeezing the mortar into the
The product reviewed in this EPD contains the borehole the fixing element has to be set within the working
following component volumes: time mentioned in the Instructions for Use. After the curing time,
described as well in the Instructions for Use, the mortar is ready
Cement-based component: to take up loads.
Cement: 70 to 80% by weight
Water: 15 to 25% by weight 2.9 Packaging
Other: < 3% by weight Hilti HIT-FP 700-R is supplied in the form of a 2-foil-pack
system and thus leads to very little waste remaining after use
Limestone-based component: on the construction site.
Calcium carbonate: 70 to 80% by weight The uncured product must be disposed of as special waste in
Water: 10 to 20% by weight accordance with official regulations.
Organic acids: < 5% by weight The outer packaging consisting of plastic foil and cardboard
Other: < 5% by weight boxes designed according to the product size can be recycled.
Packaging contaminated by the product must be disposed in a
This product article contains substances listed in the candidate safe manner in
list (date: 30.06.2022) exceeding 0.1 percentage by mass: no. accordance with local/national regulations.
This product contains other Carcinogenic, Mutagenic,
2.10 Condition of use
Reprotoxic (CMR) substances in categories 1A or 1B which are
not on the candidate list, exceeding 0.1 percentage by mass: During the installation, the temperature of the base material
no. must be between 5° C and 40° C. The
Biocide products were added to this construction product or it temperature of the product should be between 5° C and 25 °C
has been treated with biocide products (this does not concern a during storage and
treated product as defined by the (EU) Ordinance on Biocide 5° C and 40° C during usage. Hilti literature and official
Products No. 528/2012): yes (during production, below 0,01% approvals must always
by weight). be considered. The two components of HIT‑FP
700-R are only for use in combination with the defined volume
2.6 Manufacture ratio and under
3 Environmental-Product Declaration - Hilti AG - HIT-FP 700-R
the conditions mentioned above to build up a dense inorganic material, Hilti HIT-FP 700-R mortar does not contribute towards
microstructure. spreading fire.
Fire protection
2.11 Environment and health during use
Refer to the Safety Data Sheet (SDS) for detailed information Name Value
on handling, storage as well as first aid, firefighting and Building material class A1
accidental release measures and disposal considerations. Burning droplets No performance assessed
Following the given instructions helps to minimize the risk to
Smoke gas development No performance assessed
health and the environment.
2.12 Reference service life Water
Hilti HIT-FP 700-R is exposed to a wide variety of The cured product behaves similarly to regular Portland
environmental factors during the use phase. The anticipated cement-based materials. HIT-FP 700-R is certified for use as an
Reference Service Life depends on the specific installation anchoring adhesive in concrete for water treatment applications
situation and the product exposure according to National Sanitation Foundation (US) NSF.
scenario. The main factors influencing the period of use involve
weathering as well as mechanical loads and chemical Mechanical destruction
exposure. It is recommended to use dust protection during the demolition
Description of the influences on the ageing of the product when of the cured chemical anchor.
applied in accordance with the rules of technology.
2.14 Re-use phase
The product cannot be reused. After usage the product can be
2.13 Extraordinary effects removed by demolition.
Fire
2.15 Disposal
Even
without any special fire safety features the Injection Systems Uncured Hilti HIT-FP 700-R can be disposed of according to the
comply with at European waste code 08 04 09* or 20 01 27*. The built-in cured
least the requirements of the EN 13501-1 standard for fire anchor can be disposed as construction waste for which the
classes A1. During European waste code 17 01 01 applies.
the curing process of Hilti HIT-FP 700-R a dense inorganic
2.16 Further information
mictrostructure, similar to concrete, is established. This leads to
Further information is available on request under
a high fire
anchor.hse@hilti.com and on the Hilti website: www.hilti.group
resistance and extraordinary creep resistance in case of fire. As
an inorganic
3. LCA: Calculation rules
• C2, transportation,
3.1 Declared Unit • C3, waste treatment,
The declared product here is an injection mortar from HILTI AG • C4, elimination.
with the designation HIT-FP 700-R. The declared unit refers to
1 kg injectable mortar product in the mixing ratio of the two Reuse, recovery and recycling potential (D)
components required for processing. The packaging, based on In order to precisely record the indicators and environmental
1 kg injectable mortar product, is also included in the impacts of the declared unit, a total of 8 information modules
calculation at 0.100 kg. The following table shows the data of are considered. The information modules A1 to A3 describe the
the declared unit.. provision of materials, the transport to the production site and
Declared unit the production processes of the product itself.
Name Value Unit
Declared unit 1 kg
The primary products are sourced from the European Union.
For IBU core EPDs (where clause 3.6 is part of the EPD): for The transport takes place exclusively by truck. The following
average EPDs, an estimate of the robustness of the LCA flow charts illustrate the underlying production process.
values must be made, e.g. concerning variability of the
production process, geographical representativeness and the
influence of background data and preliminary products
compared to the environmental impacts caused by actual
production.
3.2 System boundary
Type of EPD: cradle to gate with options.The following
information modules are defined as system boundaries in this
study:
Production stage (A1- A3):
• A1, raw material extraction,
• A2, transport to manufacturer,
• A3, manufacture.
End of life (C1- C4):
• C1, dismantling/demolition,
4 Environmental-Product Declaration - Hilti AG - HIT-FP 700-R
Illustration 1: Information module A1 to A3 of product (part
1) 3.5 Background data
The database of the background data of the GaBi 10 and
ecoinvent 3.8 databases, to which this study also refers, is
documented under the following link. (Sphera).
3.6 Data quality
For the compilation of the life cycle assessment, specific data
were collected from the factory Kaufering, in Germany, of the
HILTI AG from the year 2022. The background data from the
/GaBi 10 database/ used is from the year 2022 and thus of high
relevance.
The mass of the different components of the reactive resin
mixture come from the information in the recipe. The data
quality is classified as appropriate.
Illustration 2: Information module A1 to A3 of product (part
3.7 Period under review
2)
As production of this product only started in 2022, no annual
average consumption can be used. The input and output flows
used in this calculation were therefore measured directly by the
manufacturer for this production process for a comparable
product.
3.8 Geographic Representativeness
Land or region, in which the declared product system is
manufactured, used or handled at the end of the product´s
lifespan: Germany
3.9 Allocation
Allocation of co-products takes place in the information
modules A1-A3.
The production waste of the injection-moulded
components is thermally recovered. The electrical and
thermal energy credits resulting therefrom are
completely charged in modules A1-A3.
Illustration 3: Information module A1 to A3 of packaging No further
allocations are made.
3.3 Estimates and assumptions
The electricity mixes and other background data are calculated
on a country-specific basis for the production processes.
Assumptions were made for certain data sets
An assumption was made for the calculation of material supply 3.10 Comparability
for a dispersant, thickener and L-(+)-tartaric acid. This Basically, a comparison or an evaluation of EPD data is only
assumption is based on manufacturer data. No assumptions or possible if all the data sets to be compared were created
restrictions were made for other formulation contents or according to EN 15804 and the building context, respectively
processes. the product-specific characteristics of performance, are taken
into account.
3.4 Cut-off criteria
The used background database has to be mentioned.
All energy and mass inputs were taken into account.The cut-off
criterion according to EN 15804 is not applied.
4. LCA: Scenarios and additional technical information
Characteristic product properties additional information can also be listed if necessary.
Information on biogenic carbon
The following technical information is a basis for the declared
No renewable raw materials are used in the product. Therefore, modules or can be used for developing specific scenarios in the
the biogenic carbon is shown as zero. The following raw context of a building assessment if modules are not declared
materials contain biogenic carbon in the packaging. (MND).
Information on describing the biogenic Carbon Content at
A5 is not declared including the disposal of the packaging
factory gate
material on the construction site, the amounts of packaging
Name Value Unit
materials included in the LCA calculations must be declared as
Packaging Cardboard Box 0,013 kg C technical scenario information for Module A5.
Packaging IfU-Lables, Paper 0,006 kg C
The following technical scenario information is required for the Information on packaging
declared modules and optional for non-declared modules.
Modules for which no information is declared can be deleted;
5 Environmental-Product Declaration - Hilti AG - HIT-FP 700-R
Name Value Unit End of life (C1-C4)
Componsite foil, PA6 0,0088 kg The product is demolished using an electric chisel. The
Clips, Aluminium 0,0022 kg electrical energy consumption for the tool is assumed to be
Connector, PBT 0,0169 kg 0.05 MJ for the declared unit. The electricity consumption is
calculated with a European electricity mix. The construction
Composite foil, PE-LD 0,0076 kg
waste is transported by truck 50 km to the waste treatment
Mixer, PP 0,0162 kg
plant. The construction waste is shredded in the waste
Mixer extension, PE-LD 0,0040 kg treatment plant and then dumped.
IfU- Labels, Paper 0,0142 kg
Name Value Unit
Cardboard box 0,0301 kg
Collected as mixed construction waste 1 kg
Crushing in the shredder 1 kg
In case a reference service life according to applicable ISO Landfilling 1 kg
standards is declared then the assumptions and in-use
conditions underlying the determined RSL shall be declared. In Reuse, recovery and/or recycling potentials (D), relevant
addition, it shall be stated that the RSL applies for the reference scenario information
conditions only. In this calculation there are no reuse, recovery and recycling
potentials. Therefore, the information module D is declared and
The same holds for a service life declared by the manufacturer. shown as zero.
Corresponding information related to in-use conditions needs
Name Value Unit
not be provided if a service life taken from the list on service life
Reuse, recovery and recycling potentials 0 kg
by BNB is declared.
6 Environmental-Product Declaration - Hilti AG - HIT-FP 700-R
5. LCA: Results
In Table 1 "Description of the system boundary", all declared modules shall be indicated with an "X"; all modules that are not declared
shall be indicated with "MND" (As default the modules B3, B4, B5 are marked as MNR – module not relevant). In the following tables,
columns can be deleted for modules that are not declared. Indicator values should be declared with three valid digits (eventually using
exponential form (e.g. 1,23E-5 = 0,0000123). A uniform format should be used for all values of one indicator.
If several modules are not declared and therefore have been deleted from the table, the abbreviations for the indicators can be
replaced by the complete names, while the readability and clear arrangement should be maintained; the legends can then be deleted.
If due to relevant data gaps, an indicator cannot be declared in a robust way, then the abbreviation “IND” (indicator not declared)
should be used for this indicator.
• 0 - calculated value is 0
• 0 - value falls under the cut-off
• 0 - assumption which exclude any flows (e.g. exported
electricity A1-A3)
• IND – in cases where the inventory does not support
the methodological approach or the calculation of the
specific indicator IND shall be used.
If no reference service life is declared (see chapter 2.13 "Reference Service Life"), the LCA results of the modules B1-B2 and B6-B7
shall refer to a period of one year. This shall then be indicated as an explanatory text below the tables. In addition, the formula for the
quantification of such B-modules over the total life cycle shall be provided.
DESCRIPTION OF THE SYSTEM BOUNDARY (X = INCLUDED IN LCA; ND = MODULE OR INDICATOR NOT DECLARED; MNR =
MODULE NOT RELEVANT)
BENEFITS
AND LOADS
CONSTRUCTION
BEYOND
PRODUCT STAGE PROCESS USE STAGE END OF LIFE STAGE
THE SYSTEM
STAGE
BOUNDARIE
S
la ire ta m w a Ry lp p u s tro p s n a rT g n iru tc a fu n a M e h t m o rf tro p s n a rTe tis e h t o t e ta g y lb m e s s A e s U e c n a n e tn ia M ria p e R tn e m e c a lp e R tn e m h s ib ru fe R y g re n e la n o ita re p Oe s u re ta w la n o ita re p Oe s u n o itc u rts n o c -e Dn o itilo m e d tro p s n a rT g n is s e c o rp e ts a W la s o p s iD -e s u e R-y re v o c e R-g n ilc y c e Rla itn e to p
A1 A2 A3 A4 A5 B1 B2 B3 B4 B5 B6 B7 C1 C2 C3 C4 D
X X X MND MND MND MND MNR MNR MNR MND MND X X X X X
RESULTS OF THE LCA - ENVIRONMENTAL IMPACT according to EN 15804+A2: 1 kg HILTI HIT-FP 700 R
Parameter Unit A1-A3 C1 C2 C3 C4 D
Global Warming Potential total (GWP-total) kg CO 2 eq 1.05E+00 5.12E-03 3.76E-03 2.6E-03 1.45E-02 0
Global Warming Potential fossil fuels (GWP-fossil) kg CO 2 eq 1.05E+00 5.12E-03 3.74E-03 2.59E-03 1.45E-02 0
Global Warming Potential biogenic (GWP-biogenic) kg CO 2 eq 0 0 0 0 0 0
Global Warming Potential luluc (GWP-luluc) kg CO 2 eq 7.09E-04 1.08E-06 2.07E-05 1.2E-05 2.67E-05 0
Depletion potential of the stratospheric ozone layer (ODP) kg CFC11 eq 1.91E-08 7.5E-14 2.22E-16 3.85E-15 3.4E-14 0
Acidification potential of land and water (AP) mol H+ eq 3E-03 1.12E-05 1.17E-05 1.34E-05 1.03E-04 0
Eutrophication potential aquatic freshwater (EP-freshwater) kg P eq 6.95E-05 1.49E-08 1.11E-08 7.43E-09 2.45E-08 0
Eutrophication potential aquatic marine (EP-marine) kg N eq 9.58E-04 2.52E-06 5.37E-06 6.11E-06 2.62E-05 0
Eutrophication potential terrestrial (EP-terrestrial) mol N eq 8.55E-03 2.65E-05 6.01E-05 6.74E-05 2.88E-04 0
Formation potential of tropospheric ozone photochemical oxidants kg NMVOC
2.24E-03 6.82E-06 1.05E-05 1.66E-05 7.97E-05 0
(POCP) eq
Abiotic depletion potential for non fossil resources (ADPE) kg Sb eq 5.43E-06 1.4E-09 3.1E-10 2.87E-09 1.48E-09 0
Abiotic depletion potential for fossil resources (ADPF) MJ 1.1E+01 9.29E-02 4.96E-02 5.06E-02 1.9E-01 0
m3 world eq
Water use (WDP) 1.44E-01 1.17E-03 3.33E-05 4.99E-04 1.59E-03 0
deprived
RESULTS OF THE LCA - INDICATORS TO DESCRIBE RESOURCE USE according to EN 15804+A2: 1 kg HILTI HIT-FP 700 R
Parameter Unit A1-A3 C1 C2 C3 C4 D
Renewable primary energy as energy carrier (PERE) MJ 1.68E+00 5.16E-02 2.82E-03 4.06E-03 2.85E-02 0
Renewable primary energy resources as material utilization
MJ 6.65E-01 0 0 0 0 0
(PERM)
Total use of renewable primary energy resources (PERT) MJ 2.34E+00 5.16E-02 2.82E-03 4.06E-03 2.85E-02 0
Non renewable primary energy as energy carrier (PENRE) MJ 8.8E+00 9.3E-02 4.97E-02 5.07E-02 1.9E-01 0
Non renewable primary energy as material utilization (PENRM) MJ 2.24E+00 0 0 0 0 0
Total use of non renewable primary energy resources (PENRT) MJ 1.1E+01 9.3E-02 4.97E-02 5.07E-02 1.9E-01 0
Use of secondary material (SM) kg 4.87E-02 0 0 0 0 0
Use of renewable secondary fuels (RSF) MJ 0 0 0 0 0 0
Use of non renewable secondary fuels (NRSF) MJ 0 0 0 0 0 0
7 Environmental-Product Declaration - Hilti AG - HIT-FP 700-R
Use of net fresh water (FW) m3 4.87E-03 4.92E-05 3.19E-06 1.42E-05 4.82E-05 0
RESULTS OF THE LCA – WASTE CATEGORIES AND OUTPUT FLOWS according to EN 15804+A2:
1 kg HILTI HIT-FP 700 R
Parameter Unit A1-A3 C1 C2 C3 C4 D
Hazardous waste disposed (HWD) kg 1.42E-08 8.04E-12 2.38E-13 6.34E-13 9.75E-12 0
Non hazardous waste disposed (NHWD) kg 3.03E-02 7E-05 7.13E-06 1.34E-05 9.71E-01 0
Radioactive waste disposed (RWD) kg 1.84E-04 1.49E-05 6.13E-08 6.68E-07 2.11E-06 0
Components for re-use (CRU) kg 0 0 0 0 0 0
Materials for recycling (MFR) kg 0 0 0 0 0 0
Materials for energy recovery (MER) kg 0 0 0 0 0 0
Exported electrical energy (EEE) MJ 0 0 0 0 0 0
Exported thermal energy (EET) MJ 0 0 0 0 0 0
RESULTS OF THE LCA – additional impact categories according to EN 15804+A2-optional:
1 kg HILTI HIT-FP 700 R
Parameter Unit A1-A3 C1 C2 C3 C4 D
Disease
Incidence of disease due to PM emissions (PM) ND ND ND ND ND ND
incidence
Human exposure efficiency relative to U235 (IR) kBq U235 eq ND ND ND ND ND ND
Comparative toxic unit for ecosystems (ETP-fw) CTUe ND ND ND ND ND ND
Comparative toxic unit for humans (carcinogenic) (HTP-c) CTUh ND ND ND ND ND ND
Comparative toxic unit for humans (noncarcinogenic) (HTP-nc) CTUh ND ND ND ND ND ND
Soil quality index (SQP) SQP ND ND ND ND ND ND
The secondary material (SM) used leads from paper production.
Disclaimer
2 – for the indicators “abiotic depletion potential for non-fossil resources”, “abiotic
depletion potential for fossil resources”, “water (user) deprivation potential,
deprivation-weighted water consumption”, “potential comparative toxic unit for
ecosystems”, “potential comparative toxic unit for humans – cancerogenic”, “Potential
comparative toxic unit for humans - not cancerogenic”, “potential soil quality
index”.
The results
of this environmental impact indicator shall be used with care as the
uncertainties
on these results are high as there is limited experience with the
indicator.
6. LCA: Interpretation
The dominance analysis shows that the main causes for the The injectable mortar mixture itself accounts for 74 % of the
environmental impacts and indicators can be found in total global warming potential in information module A1. Approx.
information module A1. This shows the total global warming 7 % is made up of the PA6 of the composite foil and approx. 6
potential for material provision at around 88 %, based on all % is made up of the Polybutylene terephthalate (PBT) of the
information modules. With the total non-renewable primary connector.
energy it is about 87 %.
Illustration: Dominance analysis A1- A3
If you look at the material provision of the injectable mortar
mixture and the packaging in detail, it becomes clear which raw Illustration: Dominance analysis A1
materials make a decisive contribution to the respective
environmental effects and indicators. Within the injectable mortar mixture itself, about 75 % of the
total global warming potential and about 42 % of the total non-
8 Environmental-Product Declaration - Hilti AG - HIT-FP 700-R
renewable primary energy are created by the material provision Illustration: Dominance analysis A1, injectable mortar
of cement. Lithium hydroxide has a share of about 6 % of the mixture
total greenhouse gas emissions and about 9 % of the total non-
renewable primary energy.
7. Requisite evidence
As a general rule, all statements must be documented with Hilti HIT-FP 700-R complies with the requirements of
measured data (presented by the corresponding test
• DIBt (2010) in combination with the NIK values from
certificates). The methods of evidence and the test conditions
AgBB (2021) for applications in interior areas
have to be described together with the results.
• emission class A+ outlined in the French VOC Directives
in accordance with the Eurofins attestation,
If substances are not detected, the limit of detection must be
• CDPH/EHLB Standard Method V 1.2 (2017)
included in the declaration.
in accordance with Eurofins test report, No. 392-2021-
00413601_A_EN and Eurofins tes report, No. 392-2021-
Interpreting statements such as “… free of …” or “… are
00413601_H_EN respectively.
entirely harmless …” are not allowed.
AgBB overview of results (28 days [µg/m³])
If evidence required by the specific PCR part B is not provided, Name Value Unit
this has to be justified under the respective title for the required TVOC (C6 - C16) < <1000 μg/m3
evidence.
Sum SVOC (C16 - C22) < <100 μg/m3
If relevant for the scope of application of the declared product, R (dimensionless) < <1 -
or if derivable from its material composition, it is recommended VOC without NIK < <100 μg/m3
to provide additional adequate evidence.
Carcinogenic Substances < <1 μg/m3
8. References
DIN EN 196-1 the product category of construction products
DIN EN 196-1: 2016-11, Prüfverfahren für Zement - Teil 1:
Bestimmung der Festigkeit ISO 14001
ISO 14001: 2015-09, Umweltmanagementsysteme -
Anforderungen mit Anleitung zur Anwendung
DIN EN 14293
DIN EN 14293: 2006-10, Klebstoffe - Klebstoffe für das Kleben
von Parkett auf einen Untergrund - Prüfverfahren und ISO 14025
Mindestanforderungen DIN EN /ISO 14025:2011-10/, Environmental labels and
declarations — Type III environmental declarations —
Principles and procedures
EN ISO 1183-3
EN ISO 1183-3: 2000-05, Kunststoffe - Bestimmung der Dichte ISO 9001
von nicht verschäumten Kunststoffen - Teil 3: Gas-Pyknometer- ISO 9001: 2015-11, Qualitätsmanagementsysteme -
Verfahren Anforderungen
EN 13501-1 ISO 50001
EN 13501-1: 2019-05, ISO 50001: 2018-08, Energiemanagementsysteme -
Klassifizierung von Bauprodukten und Bauarten zu ihrem Anforderungen mit Anleitung zur Anwendung
Brandverhalten - Teil 1: Klassifizierung mit den Ergebnissen
aus den Prüfungen zum Brandverhalten von Bauprodukten AgBB (2021)
Vorgehensweise bei der gesundheitlichen Bewertung der
Emissionen von flüchtigen organischen Verbindungen (VVOC,
EN 15804 VOC und SVOC) aus Bauprodukten (2021)
EN 15804+A2:2019+AC:2021, Sustainability of construction
works — Environmental Product Declarations — Core rules for
9 Environmental-Product Declaration - Hilti AG - HIT-FP 700-R
CDPH/EHLB/Standard Method V1.2
California CDPH Standard Method is a US standard for
evaluating and restricting VOC emissions to indoor air.
Developed in California as "Section 01350" Specification, (08.09.2022)
several systems in the US refer to CDPH Standard Method
Candidate List of substances of very high concern for
Authorisation
European Cheminals Agency (ECHA), in accordance with
Article 50(10) of the REACH regulation
IBU 2021
DIBt (2010)
Grundsätze zur gesundheitlichen Bewertung von Bauprodukten
in Innenräumen (Oktober 2010) General
Instructions for the EPD programme of Institut Bauen und
Umwelt e.V. Version
ETA-21/0624 2.0,
European Technical Approval Hilti HIT-FP 700-R
Eurofins test report, No. 392-2021-00413601_A_EN Berlin:
VOC test report for verification of compliance with Institut Bauen und Umwelt e.V.,2021
DIBt(2010)/AgBB(2021)
www.ibu-epd.de
Eurofins test report, No. 392-2021-00413601_A_EN
VOC test report for verification of compliance with the French
directive from 2010
Eurofins test report, No. 392-2021-00413601_H_EN
VOC test report for verification of compliance with Calculation rules: PCR - Part A
CDPH/EHLB/Standard Method V1.2 from 2017
European Waste code
in accordance with the European Waste Catalogue (EWC) Institut Bauen
(EWC 2014/955/EU) Commission Decision amending Decision und Umwelt e.V. (IBU), 2022. Product Category Rules for
2000/532/EC on the list of waste pursuant to Directive Building-Related
2008/98/EC of the European Products and Services. Part A: Calculation rules for the life
Parliament and of the Council cycle assessment
and requirements on the project report. Version 1.3 (08.2022)
French VOC Directives
Décret no 2011321 du 23 mars 2011 relatif à l’étiquetage des
produits de construction ou de revêtement de mur ou de sol et
des peintures et vernis sur leurs émissions de polluants volatils
Arrêté du 19 avril 2011 relatif à l’étiquetage des produits de
construction ou de revêtement de mur ou de sol et des
peintures et vernis sur leurs émissions de polluants volatils
Product category rules for construction products – Part B
NSF
NSF/ANSI/CAN 61 Drinking Water System Components Health
Effects
Reaction resin products, 01.2019
ecoinvent 3.8
Backgroun data: ecoinvent
3.8 Regulation (EU) No. 305/2011 (CPR)
Regulation (EU) No 305/2011 of the European Parliament and
of the Council of 9 March 2011 laying down harmonised
Zürich: ecoinvent conditions for the marketing of construction products and
repealing Council Directive 89/106/EEC Text with EEA
relevance
http://www.ecoinvent.org
10 Environmental-Product Declaration - Hilti AG - HIT-FP 700-R
Sphera
https://gabi.sphera.com/databases/gabi-data-search/
GaBi 10
Software: Ganzheitliche Bilanzierung, (08.09.2022)
The literature referred to in the Environmental Product
Declaration must be listed in full.Standards already fully quoted
in the EPD do not need to be listed here again.
Leinfelden-Echterdingen; The current version of PCR Part A and PCR Part B of the PCR
Sphera Solution GmbH, document on which they are based must be referenced.
11 Environmental-Product Declaration - Hilti AG - HIT-FP 700-R
Publisher
Institut Bauen und Umwelt e.V. +49 (0)30 3087748- 0
Hegelplatz 1 info@ibu-epd.com
10117 Berlin www.ibu-epd.com
Germany
Programme holder
Institut Bauen und Umwelt e.V. +49 (0)30 3087748- 0
Hegelplatz 1 info@ibu-epd.com
10117 Berlin www.ibu-epd.com
Germany
Author of the Life Cycle Assessment
FIT-Umwelttechnik GmbH 05362 72 69 474
Westerstr. 13 bertram@fit-umwelttechnik.de
38442 Wolfsburg www.fit-umwelttechnik.com
Germany
Owner of the Declaration
Hilti Aktiengesellschaft +423 234 2111
Feldkircher Strasse 100 HAGHSE@hilti.com
9494 Schaan www.hilti.com
Liechtenstein
12 Environmental-Product Declaration - Hilti AG - HIT-FP 700-R
