ENVIRONMENTAL-PRODUCT DECLARATION
as per ISO 14025 and EN 15804+A2
Owner of the Declaration Hilti Aktiengesellschaft
Publisher Institut Bauen und Umwelt e.V. (IBU)
Programme holder Institut Bauen und Umwelt e.V. (IBU)
Declaration number EPD-HIL-20230038-IBA1-EN
Issue date 10/02/2023
Valid to 09/02/2028
HIT-HY 200-A V3
Hilti AG
www.ibu-epd.com | https://epd-online.com
1. General Information
Hilti AG HIT-HY 200-A V3
Programme holder Owner of the declaration
IBU – Institut Bauen und Umwelt e.V. Hilti Aktiengesellschaft
Hegelplatz 1 Feldkircher Strasse 100
10117 Berlin 9494 Schaan
Germany Liechtenstein
Declaration number Declared product / declared unit
EPD-HIL-20230038-IBA1-EN The declared product is a HILTI injectable mortar HIT-HY 200-A V3. The
declared unit is one kilogram of reaction resin product in the mixing ratio of
the two components necessary for processing. The packaging is also
included in the calculation. The declared unit is stated in [kg].
This declaration is based on the product category rules: Scope:
Reaction resin products, 01/08/2021 This document refers to the injectable mortar HIT-HY 200-A V3 with its
(PCR checked and approved by the SVR) packaging. For the compilation of the life cycle assessment, specific data
were collected from the factory in Kaufering, Germany, of the HILTI AG.
Since the production of this product has only just started in 2022, no
Issue date annual average consumption can be used. The input and output flows
used in this calculation were therefore measured directly by the
10/02/2023
manufacturer for this production process for a comparable product.
The owner of the declaration shall be liable for the underlying information
and evidence; the IBU shall not be liable with respect to manufacturer
Valid to
information, life cycle assessment data and evidences.
09/02/2028
The EPD was created according to the specifications of EN 15804+A2. In
the following, the standard will be simplified as EN 15804 bezeichnet.
Verification
The standard EN 15804 serves as the core PCR
Independent verification of the declaration and data according to ISO
14025:2011
internally X externally
Dipl.-Ing Hans Peters
(chairman of Institut Bauen und Umwelt e.V.)
Dr. Alexander Röder Matthias Klingler,
(Managing Director Institut Bauen und Umwelt e.V.) (Independent verifier)
1 Environmental-Product Declaration - Hilti AG - HIT-HY 200-A V3
2. Product
2.1 Product description/Product definition 2.3 Technical Data
The declared product of HIT-HY 200-A V3 is a two-component The technical specifications of the products within the scope of
system. the EPD shall be listed, including the reference to the test
The resin component (component A) comprises a resin based methods/test standards for each specification.
on methacrylate as well as mineral and cement-like fillers. The
curing agent component (component B) comprises peroxide For products with CE marking, the technical specifications must
hardener, water and mineral fillers. be specified in accordance with information in the declaration of
Mixing the two components A and B in the static mixer initiates performance. The properties relevant to the product should be
the curing (hardening) reaction of both binder systems. During specified in the table below. If no information is given for
the curing phase, a very strong bond is formed between the properties, an explanation must be given in the background
organic and inorganic binder matrix. report to the EPD as to why the property is not relevant to the
The hybrid system formed during cement and resin curing product.
results in a crosslinked duromer with desired design properties
(high bond strengths within a short curing time) and particular Constructional data
long-term stability.
Name Value Unit
Composite foils are used for the two-component foil pack of
HIT-HY 200-A V3. This kind of packaging serves the following Density EN ISO 1183-1 1830 kg/m3
purposes: waste volume reduction, easy storage and transport, Compressive strength (Tcure=120h) EN
92 N/mm2
and less packaging material. ISO 604
Through legislation and increased public awareness users have Elastic modulus (pressure) EN ISO 604 2900 N/mm2
increasingly become discerned towards the use of styrene and
Tensile shear strength acc. to DIN EN not
other highly volatile components with their resulting unpleasant N/mm2
14293 relevant
odour and low flash point (flammability).
Tensile bond strength acc. to DIN EN not
The reaction resins used in all Hilti hybrid adhesives contain no N/mm2
14293 relevant
styrene, are practically odourless and have a considerably
higher flash point, i.e. higher than 100° C in comparison to 34° Hilti HIT-HY 200-A V3 displays the following
C for styrene-based characteristics:
products.
HIT-HY 200-A V3 is a premium performance injectable hybrid Performance data of the product in accordance with the
mortar with approvals for rebar connections and heavy duty declaration of performance with respect to its essential
anchoring. For the placing of the product on the market in the characteristics according to
European Union European Free Trade Association EU/EFTA) ETA 18/0972
(with the exception of Switzerland) Regulation (EU) No. ETA 18/0978
305/2011 (CPR) applies. The product needs a declaration of ETA 19/0600
performance taking into consideration the following European ETA 19/0601
Technical Approvals ETA 19/0632
ETA 18/0972 ETA 19/0665
ETA 18/0978 ICC ESR-4878
ETA 19/0600 ICC ESR-4868
ETA 19/0601
ETA 19/0632 Shelf life of 12 months:
ETA 19/0665 Substrate temperature during installation -10 to +40 °C (internal
and the CE marking. For the application and use the respective method).
national provisions apply.
Working time:
2.2 Application
-10 to -5 °C 90 min
Hilti HIT-HY 200-A V3 serves for safely securing of threaded > -5 to 0 °C 50 min
rods and postinstalled rebar connections in cracked and > 0 to +5 °C 25 min
uncracked concrete C20/25 to C50/60. HIT-HY 200-A V3 has > 5 to +10 °C 15 min
ETAs including seismic C1 and C2 performance for anchoring > 10 to +20 °C 7 min
and fire data for rebar and anchoring designs. It also holds > 20 to +30 °C 4 min
international code council (ICC) approvals for static and A-F > 30 to +40 °C 3 min
seismic designs.
Hilti HIT-HY 200-A V3 is a component of the Hilti SAFEset Curing time:
concept. Hilti SAFEset is an approved system which makes -10 to -5 °C 7 h
anchor installation an easier, safer and faster process. It > -5 to 0 °C 4 h
significantly improves the robustness of fastening and > 0 to +5 °C 2 h
dramatically reduces the possibilities of error during installation. > 5 to +10 °C 75 min
As part of SAFEset HIT-HY 200-A V3 can be installed with > 10 to +20 °C 45 min
approved Hilti Hollow Drill bits and vacuum cleaners that drill > 20 to +30 °C 30 min
and clean the hole in one step for virtually dust-free installation. > 30 to +40 °C 30 min
When used with Hilti HIT-Z rod as part of the SAFEset, no
cleaning of the borehole is required. The use of Hilti HDE 2.4 Delivery status
dispensers with the Volume Calculator app leads to no under or The product Hilti HIT-HY 200-A V3 is available in foil-packages
over fill, reducing underfilling related risks and minimizing with a total of 330 ml and 500 ml injectable mortar in the
mortar wastage. corresponding mixing ratio.
2 Environmental-Product Declaration - Hilti AG - HIT-HY 200-A V3
The manufacturing plant of HIT-HY 200-A V3, Hilti GmbH
2.5 Base materials/Ancillary materials Industriegesellschaft für Befestigungstechnik, Hiltistr. 6, 86916
Hilti HIT-HY 200-A V3 is supplied in the form of a dual Kaufering, Germany, is certified according to ISO 14001 which
component film-wrapped pack comprising a resin component defines international standards for sustainable environmental
and a curing agent component at a volume ratio of 5:1. The management. The production site is also certified in
mixing ratio of resin and curing agent components is accordance with ISO 50001 Energy Management Systems.
automatically set during the injection process. Product curing
commences directly after the components are mixed. 2.8 Product processing/Installation
The product is delivered with Instructions for Use explaining the
The product reviewed in this EPD contains the following basic steps for installation:
component volumes: 1) For safe handling the precautionary measures described in
the SDS (e.g. hand and eye protection) must be adhered to
Resin component: 2) Insert the cartridge into the red cassette
Methacrylate resin mixture: 30 to 40% by weight 3) Screw on the mixing nozzle
Mineral fillers: 40 to 50% by weight 4) Put the cassette into the dispenser system
Cement: 10 to 20% by weight 5) Discard the first trigger pulls
Other: < 5% by weight 6) Fill 2/3 of the borehole with mortar
7) Set the fixing element
Curing agent component: After mixing the components and squeezing the mortar into the
Mineral fillers: 40 to 50% by weight borehole the fixing element has to be set within the working
Aluminium oxide: 15 to 25% by weight time mentioned in Instructions for Use. After the curing time,
Water: 15 to 25% by weight described as well in Instructions for Use, the mortar is ready to
Dibenzoyl peroxide: 10 to 15% by weight take up loads.
Other: < 5% by weight
2.9 Packaging
This product article contains substances listed in the candidate Hilti HIT-HY 200-A V3 is supplied in the form of a 2-foil-pack
list (date: 15.11.2022) exceeding 0.1 percentage by mass: no. system and thus leads to very little waste remaining after use
on the construction site. After curing, the product can be
This product contains other CMR substances in categories 1A disposed of with household waste. Full or only partially emptied
or 1B which are not on the candidate list, exceeding 0.1 cartridges must be disposed of as special waste in accordance
percentage by mass: no. with official regulations.
The outer packaging consisting of plastic foil and cardboard
Biocide products were added to this construction product or it boxes designed according to the product size can be recycled.
has been treated with biocide products (this then concerns a Packaging contaminated by the product must be disposed in a
treated product as defined by the (EU) Ordinance on Biocide safe manner in accordance with local/national regulations.
Products No. 528/2012): no.
2.10 Condition of use
2.6 Manufacture During the installation the temperature of the base material
Most raw materials are sourced in Europe. The transport is must be between -10° C and +40°C. The temperature of the
exclusively by truck for the European raw materials, and by product should be between 5 - 25 °C during storage and 0 - 40°
truck and by ship for the others. C during installation. Hilti literature and official approvals must
Chemical mortars are usually two-component systems always be considered. The two components of HIT-HY 200-A
consisting of a binder and a hardener. One of the base V3 are only for use in combination with the defined volume ratio
components of the binder is the reactive resin which in the case and under the conditions mentioned above to
of HIT-HY 200-A V3 is produced in Kaufering. build up a cross-linked filled duromer.
The resin production process is a chemical reaction of the
2.11 Environment and health during use
corresponding educts to a basic resin with subsequent mixing
of the basic resin with different reactive diluents to a reactive Refer to the Safety Data Sheet (SDS) for detailed information
resin. This process is controlled and monitored by process on handling, storage as well as first aid, firefighting and
control technology. accidental release measures and disposal considerations.
The production of chemical mortars consists of a mixing Following the given
process and a filling process of the respective single instructions help to minimize the risk to health and environment.
components (binder and hardener) and their subsequent union
2.12 Reference service life
to a two-component system
Hilti HIT-HY 200-A V3 is exposed to a wide variety of
(packaging). Here as well process control technology is used to
environmental factors during the use phase. The anticipated
weigh and mix solid and liquid compounds according to the
Reference Service Life depends on the specific installation
specification. In the next step both well-mixed components run
situation and the product exposure
through an automized filling line in which each of the processed
scenario. The main factors influencing the period of use involve
masses is filled into a tubular foil bag. Finally, the single
weathering as well as mechanical loads and chemical
components are combined in one packaging unit. The two-pack
exposure.
foil bags are packed into cardboard boxes and then finally
Description of the influences on the ageing of the product when
shipped.
applied in accordance with the rules of technology.
The manufacturing plant of HIT-HY 200-A V3, Hilti GmbH
Industriegesellschaft für Befestigungstechnik, Hiltistr. 6, 86916
Kaufering, Germany, is certified according to ISO 9001. The 2.13 Extraordinary effects
guideline defines international standards for quality and
Fire
process management.
Even without any special fire safety features the Injection
Systems comply with at least the requirements of the DIN EN
2.7 Environment and health during manufacturing
13501-1 standard for fire classes E and Efl. As cross-linked
methacrylate resins do not melt or drip, the resins do not
3 Environmental-Product Declaration - Hilti AG - HIT-HY 200-A V3
contribute towards spreading fire. Apart from the common Sanitation Foundation (US) /NSF/.
combustion produces carbon monoxide and carbon
dioxide, fire gases can contain traces of methyl methacrylate, Mechanical destruction
esters, alcohol, and hydrocarbons. Due to the quantities used, It is recommended to use dust protection during the demolition
they only have a subordinate influence on the fire of the cured chemical anchor.
characteristics of a building structure in which they have been
installed. 2.14 Re-use phase
The product cannot be reused. After usage the product can be
Fire protection
removed by demolition.
Name Value
Building material class E/Efl 2.15 Disposal
Burning droplets No performance assessed Uncured Hilti HIT-HY 200-A V3 can be disposed of according to
the European waste code 08 04 09* or 20 01 27*. The built-in
Smoke gas development No performance assessed
cured anchor can be disposed as construction waste for which
the European waste code 17 01 01 applies.
Water
The cured product is chemically inert and insoluble in water. 2.16 Further information
HIT-HY Further information is available on request under
200-A V3 is certified for use as an anchoring adhesive in anchor.hse@hilti.com and on the Hilti website:
concrete for water treatment applications according to National www.hilti.group
3. LCA: Calculation rules
3.1 Declared Unit
The product
declared here is an injection mortar from HILTI AG with the
designation HIT-HY 200-A V3. The declared unit refers to 1 kg
reaction resin product in the mixing
ratio of the two components required for processing. The
packaging, based on 1 End of life
kg of reaction resin product, is also calculated at 0.114 kg. The (C1- C4):
table below
shows the data of the declared unit.
Declared unit
• C1,
Name Value Unit
dismantling/demolition,
Declared unit 1 kg
Conversion factor to 1 kg 1
For IBU core EPDs (where clause 3.6 is part of the EPD): for
• C2,
average EPDs, an estimate of the robustness of the LCA
transportation,
values must be made, e.g. concerning variability of the
production process, geographical representativeness and the
influence of background data and preliminary products
compared to the environmental impacts caused by actual
• C3, waste
production.
treatment,
3.2 System boundary
Type of
EPD: cradle to gate with options.The following information • C4,
modules are defined elimination.
as system boundaries in this study:
Production stage (A1- A3):
• A1, raw
material extraction, Reuse, recovery
and recycling potential (D)
• A2, transport
to manufacturer, In order to
precisely record the indicators and environmental impacts of
the declared unit,
a total of 8 information modules are considered. The
• A3, information modules A1 to
manufacture. A3 describe the provision of materials, the transport to the
4 Environmental-Product Declaration - Hilti AG - HIT-HY 200-A V3
production site For Dippt and Heliogen Blue L, an assumption was made for
and the production processes of the product itself. the calculation of the material supply. This assumption is based
The primary on manufacturer data. No assumptions or limitations were
products are sourced from the European made for other formulation contents or processes.
Union and Asia .Transport is by truck and
ship. The following flow charts illustrate the underlying 3.4 Cut-off criteria
production process. All energy and mass inputs were taken into account.The cut-off
criterion according to EN 15804+A2 is not applied.
3.5 Background data
The database of
the background data of the GaBi 10 and ecoinvent 3.8
databases, to which
this study also refers, is documented under the following link.
(Sphera).
3.6 Data quality
For the
compilation of the life cycle assessment,
specific data
were collected from the factory Kaufering,
in Germany, of
Illustration 1:
the HILTI AG from the year 2022. The
Information module A1 to A3 of product (part 1)
background data
from the GaBi 10 database used is
from the year 2022
and thus of high relevance.
The mass of the
different components of the reactive resin mixture come from
the information to
the recipe. The data quality is classified as appropriate.
Illustration 2:
Information module A1 to A3 of product (part 2)
3.7 Period under review
As production
of this product only started in 2022, no annual average
consumption can be
used. The input and output flows used in this calculation were
therefore
measured directly by the manufacturer for this production
process for a
comparable product.
3.8 Geographic Representativeness
Land or region, in which the declared product system is
manufactured, used or handled at the end of the product´s
lifespan: Germany
3.9 Allocation
Illustration 3: Allocation of
Information module A1 to A3 of packaging co-products takes place in the information
modules
3.3 Estimates and assumptions
A1-A3.
The electricity mixes and other background data
are calculated country-specifically for the production processes.
The production waste of the injection-moulded
5 Environmental-Product Declaration - Hilti AG - HIT-HY 200-A V3
allocations are made.
components is thermally recovered. The electrical and
3.10 Comparability
thermal energy credits resulting therefrom are Basically, a comparison or an evaluation of EPD data is only
possible if all the data sets to be compared were created
completely charged in modules A1-A3. according to EN 15804 and the building context, respectively
the product-specific characteristics of performance, are taken
into account.
The used background database has to be mentioned.
No further
4. LCA: Scenarios and additional technical information
Characteristic product properties
Information on biogenic carbon In case a reference service life according to applicable ISO
standards is declared then the assumptions and in-use
No renewable conditions underlying the determined RSL shall be declared. In
raw materials are used in the product. Therefore, the biogenic addition, it shall be stated that the RSL applies for the reference
carbon is shown conditions only.
as zero. The following raw materials contain biogenic carbon in
the packaging. The same holds for a service life declared by the manufacturer.
Corresponding information related to in-use conditions needs
Information on describing the biogenic Carbon Content at
not be provided if a service life taken from the list on service life
factury gate
by BNB is declared.
Name Value Unit
Packaging Cardboard Box 0,0154 kg C
End of life (C1-C4)
Packaging IfU-Lables, Paper 0,0101 kg C
The
product is demolished using an electric chisel. The electrical
The following technical scenario information is required for the energy
declared modules and optional for non-declared modules. consumption for the tool is assumed to be 0.05 MJ for the
Modules for which no information is declared can be deleted; declared unit. The
additional information can also be listed if necessary. electricity consumption is calculated with a European electricity
mix. The
The following technical information is a basis for the declared construction waste is transported by truck 50 km to the waste
modules or can be used for developing specific scenarios in the treatment plant.
context of a building assessment if modules are not declared The construction waste is shredded in the waste treatment
(MND). plant and then
dumped.
A5 is not declared including the disposal of the packaging
Name Value Unit
material on the construction site, the amounts of packaging
Collected as mixed construction waste 1 kg
materials included in the LCA calculations must be declared as
technical scenario information for Module A5. Crushing in the shredder 1 kg
Landfilling 1 kg
Reuse, recovery and/or recycling potentials (D), relevant
Information on packaging
scenario information
Name Value Unit
In this calculation there are no reuse, recovery and
Componsite foil PE/PET (foil bags) 0,0078 kg recycling potentials. Therefore, the information module D is
Clips, Aluminium 0,0027 kg declared and shown
Connector PE-HD 0,0123 kg as zero.
Composite foil PA/PE (outer packaging) 0,0094 kg Name Value Unit
Mixer, PP 0,0186 kg Reuse, recovery and recycling potentials 0 kg
Mixer extension, PE-LD 0,0045 kg
IfU- Labels, Paper 0,0235 kg
Cardboard box 0,0360 kg
6 Environmental-Product Declaration - Hilti AG - HIT-HY 200-A V3
5. LCA: Results
In Table 1 "Description of the system boundary", all declared modules shall be indicated with an "X"; all modules that are not declared
shall be indicated with "MND" (As default the modules B3, B4, B5 are marked as MNR – module not relevant). In the following tables,
columns can be deleted for modules that are not declared. Indicator values should be declared with three valid digits (eventually using
exponential form (e.g. 1,23E-5 = 0,0000123). A uniform format should be used for all values of one indicator.
If several modules are not declared and therefore have been deleted from the table, the abbreviations for the indicators can be
replaced by the complete names, while the readability and clear arrangement should be maintained; the legends can then be deleted.
If due to relevant data gaps, an indicator cannot be declared in a robust way, then the abbreviation “IND” (indicator not declared)
should be used for this indicator.
• 0 - calculated value is 0
• 0 - value falls under the cut-off
• 0 - assumption which exclude any flows (e.g. exported
electricity A1-A3)
• IND – in cases where the inventory does not support
the methodological approach or the calculation of the
specific indicator IND shall be used.
If no reference service life is declared (see chapter 2.13 "Reference Service Life"), the LCA results of the modules B1-B2 and B6-B7
shall refer to a period of one year. This shall then be indicated as an explanatory text below the tables. In addition, the formula for the
quantification of such B-modules over the total life cycle shall be provided.
DESCRIPTION OF THE SYSTEM BOUNDARY (X = INCLUDED IN LCA; ND = MODULE OR INDICATOR NOT DECLARED; MNR =
MODULE NOT RELEVANT)
BENEFITS
AND LOADS
CONSTRUCTION
BEYOND
PRODUCT STAGE PROCESS USE STAGE END OF LIFE STAGE
THE SYSTEM
STAGE
BOUNDARIE
S
la ire ta m w a Ry lp p u s tro p s n a rT g n iru tc a fu n a M e h t m o rf tro p s n a rTe tis e h t o t e ta g y lb m e s s A e s U e c n a n e tn ia M ria p e R tn e m e c a lp e R tn e m h s ib ru fe R y g re n e la n o ita re p Oe s u re ta w la n o ita re p Oe s u n o itc u rts n o c -e Dn o itilo m e d tro p s n a rT g n is s e c o rp e ts a W la s o p s iD -e s u e R-y re v o c e R-g n ilc y c e Rla itn e to p
A1 A2 A3 A4 A5 B1 B2 B3 B4 B5 B6 B7 C1 C2 C3 C4 D
X X X MND MND MND MND MNR MNR MNR MND MND X X X X X
RESULTS OF THE LCA - ENVIRONMENTAL IMPACT according to EN 15804+A2: 1 kg HILTI HIT-HY 200-A V3
Parameter Unit A1-A3 C1 C2 C3 C4 D
Global Warming Potential total (GWP-total) kg CO 2 eq 2.5E+00 5.12E-03 3.76E-03 2.6E-03 1.45E-02 0
Global Warming Potential fossil fuels (GWP-fossil) kg CO 2 eq 2.5E+00 5.12E-03 3.74E-03 2.59E-03 1.45E-02 0
Global Warming Potential biogenic (GWP-biogenic) kg CO 2 eq 0 0 0 0 0 0
Global Warming Potential luluc (GWP-luluc) kg CO 2 eq 1.27E-03 1.08E-06 2.07E-05 1.2E-05 2.67E-05 0
Depletion potential of the stratospheric ozone layer (ODP) kg CFC11 eq 4.41E-08 7.5E-14 2.22E-16 3.85E-15 3.4E-14 0
Acidification potential of land and water (AP) mol H+ eq 9.59E-03 1.12E-05 1.17E-05 1.34E-05 1.03E-04 0
Eutrophication potential aquatic freshwater (EP-freshwater) kg P eq 5.33E-04 1.49E-08 1.11E-08 7.43E-09 2.45E-08 0
Eutrophication potential aquatic marine (EP-marine) kg N eq 2.12E-03 2.52E-06 5.37E-06 6.11E-06 2.62E-05 0
Eutrophication potential terrestrial (EP-terrestrial) mol N eq 2.07E-02 2.65E-05 6.01E-05 6.74E-05 2.88E-04 0
Formation potential of tropospheric ozone photochemical oxidants kg NMVOC
6.6E-03 6.82E-06 1.05E-05 1.66E-05 7.97E-05 0
(POCP) eq
Abiotic depletion potential for non fossil resources (ADPE) kg Sb eq 1.76E-04 1.4E-09 3.1E-10 2.87E-09 1.48E-09 0
Abiotic depletion potential for fossil resources (ADPF) MJ 4.74E+01 9.29E-02 4.96E-02 5.06E-02 1.9E-01 0
m3 world eq
Water use (WDP) 7.06E-01 1.17E-03 3.33E-05 4.99E-04 1.59E-03 0
deprived
RESULTS OF THE LCA - INDICATORS TO DESCRIBE RESOURCE USE according to EN 15804+A2: 1 kg HILTI HIT-HY 200-A V3
Parameter Unit A1-A3 C1 C2 C3 C4 D
Renewable primary energy as energy carrier (PERE) MJ 4.96E+00 5.16E-02 2.82E-03 4.06E-03 2.85E-02 0
Renewable primary energy resources as material utilization
MJ 9.5E-01 0 0 0 0 0
(PERM)
Total use of renewable primary energy resources (PERT) MJ 5.91E+00 5.16E-02 2.82E-03 4.06E-03 2.85E-02 0
Non renewable primary energy as energy carrier (PENRE) MJ 4.52E+01 9.3E-02 4.97E-02 5.07E-02 1.9E-01 0
Non renewable primary energy as material utilization (PENRM) MJ 2.29E+00 0 0 0 0 0
Total use of non renewable primary energy resources (PENRT) MJ 4.75E+01 9.3E-02 4.97E-02 5.07E-02 1.9E-01 0
Use of secondary material (SM) kg 6.55E-02 0 0 0 0 0
Use of renewable secondary fuels (RSF) MJ 0 0 0 0 0 0
Use of non renewable secondary fuels (NRSF) MJ 0 0 0 0 0 0
7 Environmental-Product Declaration - Hilti AG - HIT-HY 200-A V3
Use of net fresh water (FW) m3 1.98E-02 4.92E-05 3.19E-06 1.42E-05 4.82E-05 0
RESULTS OF THE LCA – WASTE CATEGORIES AND OUTPUT FLOWS according to EN 15804+A2:
1 kg HILTI HIT-HY 200-A V3
Parameter Unit A1-A3 C1 C2 C3 C4 D
Hazardous waste disposed (HWD) kg 2.1E-08 8.04E-12 2.38E-13 6.34E-13 9.75E-12 0
Non hazardous waste disposed (NHWD) kg 4.34E-02 7E-05 7.13E-06 1.34E-05 9.71E-01 0
Radioactive waste disposed (RWD) kg 5.4E-04 1.49E-05 6.13E-08 6.68E-07 2.11E-06 0
Components for re-use (CRU) kg 0 0 0 0 0 0
Materials for recycling (MFR) kg 0 0 0 0 0 0
Materials for energy recovery (MER) kg 0 0 0 0 0 0
Exported electrical energy (EEE) MJ 0 0 0 0 0 0
Exported thermal energy (EET) MJ 0 0 0 0 0 0
RESULTS OF THE LCA – additional impact categories according to EN 15804+A2-optional:
1 kg HILTI HIT-HY 200-A V3
Parameter Unit A1-A3 C1 C2 C3 C4 D
Disease
Incidence of disease due to PM emissions (PM) ND ND ND ND ND ND
incidence
Human exposure efficiency relative to U235 (IR) kBq U235 eq ND ND ND ND ND ND
Comparative toxic unit for ecosystems (ETP-fw) CTUe ND ND ND ND ND ND
Comparative toxic unit for humans (carcinogenic) (HTP-c) CTUh ND ND ND ND ND ND
Comparative toxic unit for humans (noncarcinogenic) (HTP-nc) CTUh ND ND ND ND ND ND
Soil quality index (SQP) SQP ND ND ND ND ND ND
Disclaimer 2 –
for the indicators “abiotic depletion potential for non-fossil resources”,
“abiotic depletion potential for fossil resources”, “water (user) deprivation
potential, deprivation-weighted water consumption”, “potential comparative
toxic unit for ecosystems”, “potential comparative toxic unit for humans –
cancerogenic”, “Potential comparative toxic unit for humans - not
cancerogenic”, “potential soil quality index”.
The results of
this environmental impact indicator shall be used with care as the
uncertainties
on these results are high as there is limited experience with the
indicator.
6. LCA: Interpretation
The dominance analysis shows that the main causes of
environmental impacts and indicators are to be found in
information module A1. This is shown by the total global
warming potential for material supply with approx. 92%, related
to all information modules. For total non-renewable primary
energy, the figure is approx. 95%.
Illustration:
Illustration: Dominance analysis A1
Dominance analysis A1- A3
If we look at the material supply of the reaction resin mixture Within the reaction resin mixture itself, the material supply
and the packaging in detail, it becomes clear which raw of the BDDMA generates approx. 35% of the total global
materials contribute decisively to the respective environmental warming potential and approx. 36% of the total non-
impacts and indicators. renewable primary energy. The UMA 121 has a share of
approx. 27% of the total greenhouse gas emissions and
The reaction resin mixture itself has a share of 92% of the total approx. 29% of the total non-renewable primary energy.
global warming potential in information module A1. Approx. 2%
is accounted for by the PE-HD of the connector and approx. 3%
by the PP of the mixer.
8 Environmental-Product Declaration - Hilti AG - HIT-HY 200-A V3
Illustration:
Dominance analysis A1, reaction resin mixture
7. Requisite evidence
As a general rule, all statements must be documented with
• DIBt (2010) in combination with the NIK values from
measured data (presented by the corresponding test
AgBB (2021) for applications in interior areas,
certificates). The methods of evidence and the test conditions
• emission class A+ outlined in the French VOC Directives
have to be described together with the results.
(2011) in accordance with the Eurofins attestation,
• CDPH/EHLB Standard Method V 1.2 (2017)
If substances are not detected, the limit of detection must be
in accordance with Eurofins test report, No. 392-2021-
included in the declaration.
484601_C_EN, Eurofins test report, No. 392-2021-
00484601_E_EN and Eurofins test report, No. 392-2021-
Interpreting statements such as “… free of …” or “… are
00484602_H_EN respectively.
entirely harmless …” are not allowed.
AgBB overview of results (28 days [µg/m³])
If evidence required by the specific PCR part B is not provided, Name Value Unit
this has to be justified under the respective title for the required TVOC (C6 - C16) <1000 μg/m3
evidence.
Sum SVOC (C16 - C22) <100 μg/m3
If relevant for the scope of application of the declared product, R (dimensionless) <1 -
or if derivable from its material composition, it is recommended VOC without NIK <100 μg/m3
to provide additional adequate evidence.
Carcinogenic Substances <1 μg/m3
Hilti HIT-HY 200-A V3 complies with the requirements of
8. References
DIN EN 13501-1
Klassifizierung von Bauprodukten und Bauarten zu ihrem ISO 50001
Brandverhalten ISO 50001: 2018 Energy management systems Requirements
with guidance for use
DIN EN 14293
Klebstoffe - Klebstoffe für das Kleben von Parkett auf einen
Untergrund Prüfverfahren und Mindestanforderungen ISO 9001
ISO 9001: 2015-11, Qualitätsmanagementsysteme -
EN 15804 Anforderungen
EN 15804:2012+A1:2013, Sustainability of construction works
— Environmental Product Declarations — Core rules for the AgBB (2021)
product category of construction products. Vorgehensweise bei der gesundheitlichen Bewertung der
Emissionen von flüchtigen organischen Verbindungen (VVOC,
EN 15804 VOC und SVOC) aus Bauprodukten (2021)
EN 15804:2012+A2:2019, Sustainability of construction works
— Environmental Product Declarations — Core rules for the Candidate List of substances of very high concern for
product category of construction products. Authorisation
European Cheminals Agency (ECHA), in accordance with
EN ISO 1183-1 Article 50(10) of the REACH regulation
DIN 51757:2011-01 Plastics - Methods for determining the
density of non-cellular plastics - Part 1: Immersion method, CDPH/EHLB/Standard Method V1.2
liquid pyknometer method and titration method California CDPH Standard Method is a US standard for
evaluating and restricting VOC emissions to indoor air.
EN ISO 604 Developed in California as "Section 01350" Specification,
DIN EN ISO 604:2003-12: Determination of compressive several systems in the US refer to
properties CDPH Standard Method
ISO 14001 DIBt (2010)
ISO 14001:2015 Environmental management systems Grundsätze zur gesundheitlichen Bewertung von Bauprodukten
Requirements in Innenräumen (Oktober 2010)
with guidance for use Eurofins test report, No. 392-2021-00484601_C_EN VOC test
9 Environmental-Product Declaration - Hilti AG - HIT-HY 200-A V3
report for verification of compliance with
DIBt(2010)/AgBB(2021) Backgroun data:
ecoinvent 3.8
Eurofins test report, No. 392-2021-00484601_E_EN
VOC test report for verification of compliance with the French
VOC directive from 2011
Zürich:
Eurofins test report, No. 392-2021-00484602_H_EN ecoinvent
VOC test report for verification of compliance with
CDPH/EHLB/Standard Method V1.2 (2017)
European Waste code http://www.ecoinvent.org
in accordance with the European Waste Catalogue (EWC)
(EWC 2014/955/EU) Commission Decision amending Decision
2000/532/EC on the list of waste pursuant to Directive
2008/98/EC of the European (21.11.2022)
Parliament and of the Council
IBU 2021
ETA 18/0972
European Technical Approval Hilti HIT-HY 200-A V3 and Hilti
HIT-HY 200-R V3
General
ETA 18/0978 Instructions for the EPD programme of Institut Bauen und
European Technical Approval Hilti HIT-HY 200-A V3 and Hilti Umwelt e.V. Version
HIT-HY 200-R V3 2.0,
ETA 19/0600
European Technical Approval Hilti HIT-HY 200-A V3 and Hilti Berlin:
HIT-HY 200-R V3 Institut Bauen und Umwelt e.V.,2021
ETA 19/0601
European Technical Approval Hilti HIT-HY 200-A V3 and Hilti
HIT-HY 200-R V3 www.ibu-epd.de
Calculation rules: PCR - Part A
ETA-19/0632
European Technical Approval Hilti HIT-HY 200-A V3 and Hilti
HIT-HY 200-R V3
Institut Bauen
ETA 19/0665 und Umwelt e.V. (IBU), 2022. Product Category Rules for
European Technical Approval Hilti HIT-HY 200-A V3 and Hilti Building-Related
HIT-HY 200-R V3 Products and Services. Part A: Calculation rules for the life
cycle assessment
and requirements on the project report. Version 1.3 (08.2022)
French VOC Directives Product category rules for construction products – Part B
Décret no 2011-321 du 23 mars 2011 relatif à l’étiquetage des
produits de construction ou de revêtement de mur ou de sol et
des peintures et vernis sur leurs émissions de polluants volatils
Arrêté du 19 avril 2011 relatif à l’étiquetage des produits de Reaction resin
construction ou de revêtement de mur ou de sol et des products, 07.2014
peintures et vernis sur leurs émissions de polluants volatils Regulation (EU) No. 305/2011 (CPR)
Regulation (EU) No 305/2011 of the European Parliament and
of the Council of 9 March 2011 laying down harmonised
ICC ESR-4878 conditions for the marketing of construction products and
International code council (ICC), Evaluation report ESR-4878 repealing Council Directive 89/106/EEC Text with EEA
HILTI HIT-HY 200 V3 (November 2021) relevance
Sphera
ICC ESR-4868 GaBi 10
International code council (ICC), Evaluation report ESR-4868 Software: Ganzheitliche Bilanzierung,
HILTI HIT-HY 200 V3 (March 2022) Leinfelden-Echterdingen;
Sphera Solution GmbH,
NSF https://gabi.sphera.com/databases/gabi-data-search/
NSF/ANSI/CAN 61 Drinking Water System Components -
Health
Effects
ecoinvent 3.8
10 Environmental-Product Declaration - Hilti AG - HIT-HY 200-A V3
in the EPD do not need to be listed here again.
(21.11.2022) The current version of PCR Part A and PCR Part B of the PCR
The literature referred to in the Environmental Product document on which they are based must be referenced.
Declaration must be listed in full.Standards already fully quoted
11 Environmental-Product Declaration - Hilti AG - HIT-HY 200-A V3
Publisher
Institut Bauen und Umwelt e.V. +49 (0)30 3087748- 0
Hegelplatz 1 info@ibu-epd.com
10117 Berlin www.ibu-epd.com
Germany
Programme holder
Institut Bauen und Umwelt e.V. +49 (0)30 3087748- 0
Hegelplatz 1 info@ibu-epd.com
10117 Berlin www.ibu-epd.com
Germany
Author of the Life Cycle Assessment
FIT-Umwelttechnik GmbH 05362 72 69 474
Westerstr. 13 bertram@fit-umwelttechnik.de
38442 Wolfsburg www.fit-umwelttechnik.com
Germany
Owner of the Declaration
Hilti Aktiengesellschaft +423 234 2111
Feldkircher Strasse 100 HAGHSE@hilti.com
9494 Schaan www.hilti.com
Liechtenstein
12 Environmental-Product Declaration - Hilti AG - HIT-HY 200-A V3
