ENVIRONMENTAL PRODUCT DECLARATION
as per ISO 14025 and EN 15804+A2
Owner of the Declaration Kronospan Luxembourg S.A.
Publisher Institut Bauen und Umwelt e.V. (IBU)
Programme holder Institut Bauen und Umwelt e.V. (IBU)
Declaration number EPD-KRO-20230156-CBA1-EN
Issue date 11.07.2023
Valid to 10.07.2028
High Density Fibreboard (HDF)
Kronospan Luxembourg S.A.
www.ibu-epd.com | https://epd-online.com
General Information
Kronospan Luxembourg S.A. High Density Fibreboard (HDF)
Programme holder Owner of the declaration
IBU – Institut Bauen und Umwelt e.V. Kronospan Luxembourg S.A.
Hegelplatz 1 Rue GadderScheier 1
10117 Berlin 4984 Soleuvre
Germany Luxembourg
Declaration number Declared product / declared unit
EPD-KRO-20230156-CBA1-EN 1m3 Kronospan HDF panel
This declaration is based on the product category rules: Scope:
Wood-based panels, 01.08.2021 This document applies to Kronospan HDF panel, which is composed of
(PCR checked and approved by the SVR) wood shavings, mixed with a resin (melamine urea formaldehyde – MUF).
The declared unit weight is 870 kg/m3. LCA data were compiled using
foreground data collected based on billing documents and material
Issue date balances for the period between October 2020 and March 2022. The
declaration holder is responsible for the underlying data and its verification.
11.07.2023
The owner of the declaration shall be liable for the underlying information
and evidence; the IBU shall not be liable with respect to manufacturer
information, life cycle assessment data and evidences.
Valid to
10.07.2028 The EPD was created according to the specifications of EN 15804+A2. In
the following, the standard will be simplified as EN 15804.
Verification
The standard EN 15804 serves as the core PCR
Independent verification of the declaration and data according to ISO
14025:2011
internally X externally
Dipl.-Ing. Hans Peters
(Chairman of Institut Bauen und Umwelt e.V.)
Florian Pronold Mr Olivier Muller,
(Managing Director Institut Bauen und Umwelt e.V.) (Independent verifier)
1 Environmental Product Declaration - Kronospan Luxembourg S.A. - High Density Fibreboard (HDF)
Product
Performance data of the product in accordance with the
Product description/Product definition declaration of performance with respect to its essential
HDF (High Density Fibreboard) is engineered wood products characteristics according to EN13986:2004 + A1:2015 Wood-
that consist of panels made from a combination of wood fibres based panels for use in construction. Characteristics,
and resin. They are applicable particularly in furniture such as evaluation of conformity and marking.
doors, construction such as mouldings and indoor products
such as laminate flooring. It is especially suitable for further Base materials/Ancillary materials
finishing (routing, milling, lacquering, laminating and foiling) and The HDF panels are made of 80 - 90% of vigin wood, 8 - 18%
a good substitute for solid wood. of melamine urea formaldehyde resin (MUF), and 2% of other
The Kronobuild® product line includes HDF. For the placing on additives.
the market of the product in the European Union/European
Free Trade Association (EU/EFTA) (with the exception of This product contains substances listed in the candidate list
Switzerland) Regulation (EU) No. 305/2011 (CPR) applies. The (date: 28/02/2023) exceeding 0.1 percentage by mass : NO.
product needs a declaration of performance taking into
consideration EN 13986:2004 + A1:2015, Wood-based panels Reference service life
for use in construction - Characteristics, evaluation of The service life is assumed to be 50 years, as HDF is a non-
conformity and marking - and the CE-marking. For the structural element of a building.
application and use the respective national provisions apply
Since no use impacts are quantified (the products do not
Application require energy, maintenance or other reparation process during
Due to their homogeneous structure, HDF boards can be milled its use), this lifetime parameter does not influence the results.
three-dimensionally and then painted, foil wrapped or faced
with a paper decor in a membrane press.
The main applications HDF include interior design, furniture
components, decorative features, laminate flooring, cladding,
partitions, areas that require protection from moisture, skirting
boards / architrave and window boards / sills.
Technical Data
Technical product groups covered in this EPD are HDF.
Technical specification accounts for thicknesses of boards
within the range of 5,5 - 38mm.
Constructional data
Name Value Unit
830 -
Gross density kg/m3
890
4.62 -
Grammage kg/m2
10.15
Bending strength (longitudinal) 30 - 50 N/mm2
Bending strength (transverse) 30 - 50 N/mm2
2700 -
E-module (longitudinal) N/mm2
4800
2700 -
E-module (transverse) N/mm2
4800
Material dampness at delivery 4 - 11 %
0.5 -
Tensile strength rectangular N/mm2
0.65
0.12 -
Thermal conductivity W/(mK)
0.16
Water vapour diffusion resistance factor (wet 15.7 -
-
cup µ)* 22.9
Sound absorption coefficient (frequency range
0.2 %
1000-2000 Hz)*
Formaldehyde emissions E1 acc. to EN 717-1
or E1 DE 2020 ChemVerbotsV (E05) or TSCA - μg/m3
Title VI / CARB P2
LCA: Calculation rules
Declared unit and mass reference
Declared Unit
This declaration applies to 1 m3 of Kronospan HDF panel, with
a declared unit weight of 889.3 kg/m3.
2 Environmental Product Declaration - Kronospan Luxembourg S.A. - High Density Fibreboard (HDF)
Name Value Unit Type of EPD: Cradle-to-grave (with options)
Declared unit 1 m3 The system boundaries of the EPD follow the modular
construction system as described by EN 15804.
Mass reference 889.3 kg/m3
Layer thickness 0.0095 m The LCA considers the following modules:
Foreground data for the production processes (A1-A3) were
A1-A3: Manufacturing of pre-products, packaging, ancillary
collected from the Kronospan production site (Sanem,
materials, transport to the factory and production, with the
Luxembourg) and are and representative for the period of
associated energy supply and waste handling
October 2020 to March 2022. The manufacturing data are
A4: Transport to the construction site
specific to the technologies used in the plant and representative
A5: Installation into the building including disposal of packaging
of the local geographical context. Market share data specific to
C1: Deconstruction (screws disposal and electricity from the
each product category from the year 2021 were used to model
screwdriver)· C2: Transport to disposal sites
the transport to building site (module A4).
C3: Final product waste disposal for reuse, recycling and
energy recovery
For the further life cycle stages (modules A5 to D), generic
C4: Waste disposal, namely incineration and landfill
inventory data are used.
D: Potential for reuse, recovery and/or recycling including
These processes are not specific to Kronospan products and
benefits for product incineration from module C4
reference data or statistics were applied. The inputs of outputs
of these processes were mainly based on the COFIDAB report
Geographic Representativeness
prepared by FCBA (2012) and associated French EPD ('FDES')
Land or region, in which the declared product system is
published by FCBA. The shares between various disposal
manufactured, used or handled at the end of the product´s
routes for packaging waste (module A5) were based on
lifespan: Luxembourg
European statistics for the year 2019.
The ecoinvent database version 3.8 was used to model Comparability
background data. The average dataset based on European
Basically, a comparison or an evaluation of EPD data is only
data is used to model the glue production (no specific supplier
possible if all the data sets to be compared were created
data used).
according to EN 15804 and the building context, respectively
the product-specific characteristics of performance, are taken
System boundary
into account.
LCA: Scenarios and additional technical information
The refence service life does not affect the results since no use
Characteristic product properties of biogenic carbon impacts are quantified.
Information on describing the biogenic Carbon Content at End of life (C1-C4)
factory gate
Name Value Unit
Name ValueUnit
Collected as mixed construction waste 889.3 kg
kg
Biogenic carbon content in product 368 Energy recovery 738.1 kg
C
Landfilling 151.2 kg
Biogenic carbon content in accompanying kg
16.5
packaging C Reuse, recovery and/or recycling potentials (D), relevant
scenario information
Name Value Unit
Transport to the building site (A4) Avoided energy from incineration 10326 MJ
Name Value Unit
Transport distance (truck) 370 km
Gross density of products transported 901.2 kg/m3
Installation into the building (A5)
Name Value Unit
Auxiliary (screw) 2.54 kg
Electricity consumption 0.106 kWh
Material loss 71.1 kg
Product loss to incineration 83 %
Product loss to landfill 17 %
Packaging waste 12.9 kg
3 Environmental Product Declaration - Kronospan Luxembourg S.A. - High Density Fibreboard (HDF)
LCA: Results
The results displayed below apply to 1 m3 of Kronospan HDF panel, with a declared unit weight of 889.3 kg/m3.
DESCRIPTION OF THE SYSTEM BOUNDARY (X = INCLUDED IN LCA; ND = MODULE OR INDICATOR NOT DECLARED; MNR =
MODULE NOT RELEVANT)
Benefits and
Construction loads beyond
Product stage Use stage End-of-life stage
process stage the system
boundaries
la ire ta m w a Ry lp p u s tro p s n a rT g n iru tc a fu n a M e h t m o rf tro p s n a rTe tis e h t o t e ta g y lb m e s s A e s U e c n a n e tn ia M ria p e R tn e m e c a lp e R tn e m h s ib ru fe R y g re n e la n o ita re p Oe s u re ta w la n o ita re p Oe s u n o itc u rts n o c -e Dn o itilo m e d tro p s n a rT g n is s e c o rp e ts a W la s o p s iD -e s u e R-y re v o c e R-g n ilc y c e Rla itn e to p
A1 A2 A3 A4 A5 B1 B2 B3 B4 B5 B6 B7 C1 C2 C3 C4 D
X X X X X MND MND MNR MNR MNR MND MND X X X X X
RESULTS OF THE LCA - ENVIRONMENTAL IMPACT according to EN 15804+A2: 1 m3 Kronospan HDF panel
Parameter Unit A1-A3 A4 A5 C1 C2 C3 C4 D
GWP-total kg CO 2 eq -9.77E+02 7.63E+01 1.22E+02 4.31E-02 7.4E+00 0 1.37E+03 -3.09E+02
GWP-fossil kg CO 2 eq 4.86E+02 7.62E+01 6.61E+00 4.17E-02 7.39E+00 0 8.03E+00 -3.09E+02
GWP-biogenic kg CO 2 eq -1.47E+03 7.76E-02 1.15E+02 1.31E-03 6.65E-03 0 1.36E+03 -5.73E-02
GWP-luluc kg CO 2 eq 2.65E+00 2.74E-02 4.57E-03 9.86E-05 2.9E-03 0 2.71E-03 -9.66E-03
ODP kg CFC11 eq 5.7E-05 1.82E-05 5.28E-07 2.1E-09 1.71E-06 0 1.26E-06 -4.33E-05
AP mol H+ eq 2.72E+00 3.18E-01 4.64E-02 2.37E-04 3E-02 0 2.39E-01 -3.98E-01
EP-freshwater kg P eq 2.93E-02 5.21E-04 2.65E-04 4.46E-06 5.18E-05 0 1.36E-04 -2.82E-04
EP-marine kg N eq 4.3E-01 9.61E-02 1.6E-02 3.03E-05 8.94E-03 0 1.16E-01 -1.44E-01
EP-terrestrial mol N eq 6.25E+00 1.06E+00 1.71E-01 3.49E-04 9.87E-02 0 1.27E+00 -1.58E+00
kg NMVOC
POCP 2.37E+00 3.41E-01 5.46E-02 9.58E-05 3.02E-02 0 3.38E-01 -5.42E-01
eq
ADPE kg Sb eq 5.95E-03 1.75E-04 6.96E-05 3.86E-07 2.57E-05 0 2.88E-05 -1.82E-04
ADPF MJ 8.22E+03 1.19E+03 7.36E+01 8.84E-01 1.12E+02 0 1.03E+02 -4.31E+03
m3 world eq
WDP 6.21E+02 4.09E+00 1.49E+00 1.04E-02 3.35E-01 0 2.31E+00 -1.76E+00
deprived
GWP = Global warming potential; ODP = Depletion potential of the stratospheric ozone layer; AP = Acidification potential of land and water; EP =
Eutrophication potential; POCP = Formation potential of tropospheric ozone photochemical oxidants; ADPE = Abiotic depletion potential for non-fossil
resources; ADPF = Abiotic depletion potential for fossil resources; WDP = Water (user) deprivation potential)
RESULTS OF THE LCA - INDICATORS TO DESCRIBE RESOURCE USE according to EN 15804+A2: 1 m3 Kronospan HDF panel
Parameter Unit A1-A3 A4 A5 C1 C2 C3 C4 D
PERE MJ 2.34E+02 1.51E+01 5.59E+00 1.77E-01 1.57E+00 0 1.03E+04 0
PERM MJ 2.26E+04 0 0 0 0 0 -1.03E+04 0
PERT MJ 2.28E+04 1.51E+01 5.59E+00 1.77E-01 1.57E+00 0 0 0
PENRE MJ 8.91E+03 1.26E+03 7.8E+01 9.28E-01 1.19E+02 0 1.11E+02 -4.78E+03
PENRM MJ 0 0 0 0 0 0 0 0
PENRT MJ 8.91E+03 1.26E+03 7.8E+01 9.28E-01 1.19E+02 0 1.11E+02 -4.78E+03
SM kg 0 0 0 0 0 0 0 0
RSF MJ 6.87E+03 0 0 0 0 0 0 1.03E+04
NRSF MJ 0 0 0 0 0 0 0 0
FW m3 1.92E+01 5.9E-01 1.45E-01 1.48E-02 6.89E-02 0 4.56E-01 -2.45E-01
PERE = Use of renewable primary energy excluding renewable primary energy resources used as raw materials; PERM = Use of renewable primary
energy resources used as raw materials; PERT = Total use of renewable primary energy resources; PENRE = Use of non-renewable primary energy
excluding non-renewable primary energy resources used as raw materials; PENRM = Use of non-renewable primary energy resources used as raw
materials; PENRT = Total use of non-renewable primary energy resources; SM = Use of secondary material; RSF = Use of renewable secondary fuels;
NRSF = Use of non-renewable secondary fuels; FW = Use of net fresh water
RESULTS OF THE LCA – WASTE CATEGORIES AND OUTPUT FLOWS according to EN 15804+A2:
1 m3 Kronospan HDF panel
Parameter Unit A1-A3 A4 A5 C1 C2 C3 C4 D
HWD kg 1.31E-02 2.88E-03 3.59E-04 6.72E-07 2.92E-04 0 2.41E-04 -5.79E-03
NHWD kg 7.33E+01 1.11E+02 2.01E+01 3.09E-03 5.75E+00 0 1.56E+02 -2.36E+00
RWD kg 1.57E-02 8.04E-03 2.24E-04 6.47E-06 7.56E-04 0 3.81E-04 -4.9E-04
CRU kg 0 0 0 0 0 0 0 0
MFR kg 0 0 0 0 0 0 0 0
MER kg 0 0 7.11E+01 0 0 0 7.38E+02 0
EEE MJ 0 0 0 0 0 0 0 0
EET MJ 0 0 1.16E+03 0 0 0 1.03E+04 0
4 Environmental Product Declaration - Kronospan Luxembourg S.A. - High Density Fibreboard (HDF)
HWD = Hazardous waste disposed; NHWD = Non-hazardous waste disposed; RWD = Radioactive waste disposed; CRU = Components for re-use;
MFR = Materials for recycling; MER = Materials for energy recovery; EEE = Exported electrical energy; EET = Exported thermal energy
RESULTS OF THE LCA – additional impact categories according to EN 15804+A2-optional:
1 m3 Kronospan HDF panel
Parameter Unit A1-A3 A4 A5 C1 C2 C3 C4 D
Disease
PM 7.95E-05 8.95E-06 6.68E-07 6.54E-10 6.36E-07 0 2.08E-06 -1.24E-06
incidence
IR kBq U235 eq 1.18E+01 5.15E+00 1.92E-01 7.84E-03 4.85E-01 0 3.01E-01 -4.05E-01
ETP-fw CTUe 1.15E+04 9.28E+02 1.88E+02 5.59E-01 8.72E+01 0 1.85E+02 -3.47E+02
HTP-c CTUh 7.99E-07 2.57E-08 6E-08 1.72E-11 2.82E-09 0 2.2E-07 -1.86E-08
HTP-nc CTUh 1.05E-05 1.02E-06 2.41E-07 5.49E-10 9.14E-08 0 6.71E-07 -9.74E-07
SQP SQP 4.87E+04 1.36E+03 3.74E+01 1.6E-01 7.68E+01 0 1.09E+02 -8.44E+01
PM = Potential incidence of disease due to PM emissions; IR = Potential Human exposure efficiency relative to U235; ETP-fw = Potential comparative
Toxic Unit for ecosystems; HTP-c = Potential comparative Toxic Unit for humans (cancerogenic); HTP-nc = Potential comparative Toxic Unit for humans
(not cancerogenic); SQP = Potential soil quality index
Disclaimer 1 – for the indicator “Potential Human exposure efficiency relative to U235”. This impact category deals mainly with the
eventual impact of low-dose ionizing radiation on human health of the nuclear fuel cycle. It does not consider effects due to possible
nuclear accidents, occupational exposure or radioactive waste disposal in underground facilities. Potential ionizing radiation from the
soil, radon and from some construction materials is also not measured by this indicator.
Disclaimer 2 – for the indicators “abiotic depletion potential for non-fossil resources”, “abiotic depletion potential for fossil resources”,
“water (user) deprivation potential, deprivation-weighted water consumption”, “potential comparative toxic unit for ecosystems”,
“potential comparative toxic unit for humans – cancerogenic”, “Potential comparative toxic unit for humans - not cancerogenic”,
“potential soil quality index”. The results of this environmental impact indicator shall be used with care as the uncertainties on these
results are high as there is limited experience with the indicator.
References
Standards produits bois. Convention DHUP/CSTB 2009 Action 33 – Sous
action 5. ACV & Déclarations environnementales pour des
EN 15804 produits et composants de la construction bois.
EN 15804:2012+A2:2019+AC:2021, Sustainability of
construction works — Environmental Product Declarations — FCBA (2019)
Core rules for the product category of construction products. Fiche de déclaration environmentale et sanitaire (FDES) –
Panneaux de lamelles de bois minces orientées OSB (oriented
ISO 14025 strand board) de type 3 (panneaux travaillants utilisés en milieu
EN ISO 14025:2011, Environmental labels and declarations — humide) bruts. Epaisseur déclarée : 18 mm. FDES collective 2-
Type III environmental declarations — Principles and 90 :2018.
procedures.
FCBA (2022a)
EN 13986 Fiche de déclaration environmentale et sanitaire (FDES) –
EN 13986:2004 + A1:2015 Wood-based panels for use in Panneaux de lamelles de bois minces orientées OSB (oriented
construction - Characteristics, evaluation of conformity and strand board) de type 3 (panneaux travaillants utilisés en milieu
marking humide) bruts. Epaisseur déclarée : 12 mm. FDES collective
132289692502022.
Further References
FCBA (2022b)
PCR 2021, Part A Fiche de déclaration environmentale et sanitaire (FDES) –
PCR Guidance-Texts for Building-Related Products and Panneaux de fibres MDF (medium-density fibrebord) utilisés en
Services: Calculation Rules for the Life Cycle Assessment and milieu humide bruts. Epaisseur déclarée : 18 mm.
Requirements on the Project Report according to EN FDES collective 182289782502022.
15804+A2:2019
FCBA (2022c)
PCR 2019, Part B Fiche de déclaration environmentale et sanitaire (FDES) –
PCR-Guidances-Texts for Building-Related Products and Panneaux de fibres MDF (medium-density fibrebord) utilisés en
Services. Part B: Requirements on the EPD for Wood based milieu humide bruts. Epaisseur déclarée : 19 mm. FDES
panels collective 341289752502022.
FCBA (2012) SimaPro software and ecoinvent database:2021
Rapport d'étude Volet 2 – Prise en compte de la fin de vie des SimaPro software ecoinvent database, version 3.8, 2021
5 Environmental Product Declaration - Kronospan Luxembourg S.A. - High Density Fibreboard (HDF)
Publisher
Institut Bauen und Umwelt e.V. +49 (0)30 3087748- 0
Hegelplatz 1 info@ibu-epd.com
10117 Berlin www.ibu-epd.com
Germany
Programme holder
Institut Bauen und Umwelt e.V. +49 (0)30 3087748- 0
Hegelplatz 1 info@ibu-epd.com
10117 Berlin www.ibu-epd.com
Germany
Author of the Life Cycle Assessment
Luxembourg Institute of Science and Technology 00352-275888-1
(LIST) info@list.lu
Avenue des Hauts-Fourneaux 5 www.list.lu
4362 Esch/Alzette
Luxembourg
Owner of the Declaration
Kronospan Luxembourg S.A. +352590311214
Rue GadderScheier 1 j.guerlot@kronospan.lu
4984 Soleuvre www.kronospan.lu
Luxembourg
6 Environmental Product Declaration - Kronospan Luxembourg S.A. - High Density Fibreboard (HDF)
