Hot-rolled ribbed steel proceeding from an electric arc furnace
Environmental Product Declaration
EN ISO 14025:2010 / UNE 36904-1:2018 / EN 15804:2012+A2:2019
Hot-rolled ribbed steel
proceeding from an
electric arc furnace
Issuing date: 04/09/2023
Expiry date: 03/09/2028
The declared validity is subject to registration and publication
on www.aenor.com
Código de registro: GlobalEPD 001-007
1
Hot-rolled ribbed steel proceeding from an electric arc furnace
ÍNDICE
Limits to the system, scenarios and
1 4
General information p.4 additional technical information. p.12
1.1. The organisation p.4
1.2. Scope of the declaration p.5
1.3. Life cycle and compliance p.5
Declaration of the environmental
1.4. Differences when comparing with previous versions 5
parameters of LCA and LCI p.16
of the present EPD p.6
5.1. Environmental impact parameters p.16
5.2. Use of resources p.17
2
The product p.7 5.3. Categories of wastes p.19
5.4. Output flows p.20
2.1. Product identification p.7
2.2. Product composition p.7
2.3. Product characteristics p.8
6
Additional environmental information p.21
3
Information relative to LCA p.9
6.1. Emissions to indoor air p.21
6.2. Emissions to soil and water p.21
3.1. Life cycle assessment p.9 6.3. Biogenic carbon content p.21
3.2. Scope of the study p.9
3.3. Declared unit p.10
3.4. Allocation criteria p.10
3.5. Cut-off rule p.10 7
References
3.6. Representativeness, quality p.22
and selection of data p.11
2
Hot-rolled ribbed steel proceeding from an electric arc furnace
The declaration holder is responsible for the content and, throughout the AENOR is a founding member of ECO Platform, the European Association of
period of validity, for keeping the supporting documentation that justifies the Environmental Product Declaration Verification Programs.
data and statements included.
Declaration Holder LCA study Program administrator:
GlobalEPD
Metalúrgica Galaica S.A. Abaleo S.L.
Ctra. de Castilla, 802-820 D. José Luis Canga Cabañes. c/ Poza AENOR Internacional S.A.U.
15570 Narón – (España) de la Sal, 8; 3º A. 28031 Madrid, España C/ Génova 6.28009 Madrid, España.
(+34)9 981 399 000 (+34) 639 901 043 (+34) 902 102 201
info@megasa.com jlcanga@abaleo.es / info@abaleo.es aenordap@aenor.com
www.megasa.com www.abaleo.es www.aenor.com
UNE 36904-1:2018 Independent verification of the declaration and data in Verification body:
accordance with the EN ISO 14025:2010 Standard
The European EN 15804:2012+A2:2019 Standard
serves as the basis for the PCR.
Interna Externa
3
Hot-rolled ribbed steel proceeding from an electric arc furnace
1
GENERAL INFORMATION
1.1. The organisation
SN Seixal, Siderurgia Nacional, S.A.
The MEGASA GROUP is a family business specializing in the production and distribu- SN Seixal, Siderurgia Nacional, S.A. located in the surroundings of Lisbon, specializes
tion of long steel products. in the manufacture of ribbed products, wire rod of low, medium and high carbon,
and steel fabric. Thanks to its flexibility, it can offer ribbed steel products in different
The Group has more than a thousand employees, distributed among its different pro- presentations: bar, wild coil and spool.
duction plants and distribution units in the Iberian Peninsula and France.
With an installed capacity of more than three million tonnes, MEGASA uses an electric
SN Maia Siderurgia Nacional, S.A.
arc furnace to produce a wide range of long steels: ribbed round, wire rod, elec-
trowelded mesh and merchant and structural sections. SN Maia produces steel rebar.
The factory is located in Maia, near the city of Oporto (Portugal) and 15 km from the
port of Leixoes. It is the large factory of the group for what refers to the production
of steel rebars.
Megasa Siderúrgica, S.L.
Founded in 1953, it is located in Narón, northwest of the province of A Coruña (Spain)
in a strategic geographical position, just 9 km from the port of Ferrol. It produces
ribbed steel in bar and wild coil with a wide range of grades.
Megasider Zaragoza, S.A.U.
In 2016, Megasider Zaragoza, S.A.U. joined the Megasa Group. Recently relocated
to the outskirts of the city, it is in a strategic logistics situation in the northeast of the
Iberian Peninsula with very good communications with the most outstanding industrial
areas of the country, as well as with France.
This factory specializes in the production of merchant sections, with a wide range
of dimensions and grades. It completes its offer with ribbed products and structural
sections.
4
HHoott--rroolllleedd rriibbbbeedd sstteeeell pprroocceeeeddiinngg ffrroomm aann eelleeccttrriicc aarrcc ffuurrnnaaccee
1.2. Scope of the declaration
This environmental product declaration describes environmental information relating
to the life cycle of cradle-to-door production with options of the hot-rolled ribbed
steel made from electric arc furnace by the MEGASA GROUP in its factories of:
Carretera de Castilla, 802-820 - 15570 Narón (Spain)
Avenida de José López Soriano, 100, 50007, Zaragoza, (Spain)
Rua Siderurgia s/n, 4425-514 S. Pedro Fins, Maia (Portugal)
Rua Independência Nacional 10, 2840-996 Aldeia de Paio Pires, Seixal, (Portugal)
The role played by the product system under study is the production of hot-rolled steel
in the Seixal plant (Portugal) for use as a structural element in the construction sector.
1.3. Life cycle and compliance
The EPD has been developed and verified in accordance with the UNE-EN ISO
14025:2010, UNE-EN 36904-1 and UNE-EN 15804:2012+A2:2019 Standards.
Iron and Steel industry. Environmental Product Decla-
Heading rations. Product Category Rules. Steel products for
structures. Part 1: Basic products.
Register / Version UNE-EN 36904-1
Issuing date 2018
Administrator AENOR
5
Hot-rolled ribbed steel proceeding from an electric arc furnace
The EPD includes the life cycle stages indicated in Table 1-2. The EPD is of the cradle-
to-door type with options.
System limits. Information modules considered
A1 Supply of raw materials X
Etapa de producto A2 Transport to factory X
A3 Manufacturing X
A4 Transport to construction site X
Construcción
A5 Installation / construction MNE
B1 Use MNE The EPD may not be comparable to those developed in other Programs or in ac-
B2 Maintenance MNE cordance with other reference documents; in particular, it may not be comparable
to Declarations not developed and verified in accordance with the UNE-EN 15804
B3 Repairing MNE
Standard.
Etapa de uso B4 Replacement MNE
B5 Rehabilitation MNE Similarly, EPDs may not be comparable if the data source is different (e.g.,
databases), not all relevant information modules are included, or they are not based
B6 Energy use in service MNE
on the same scenarios.
B7 Water use in service MNE
C1 Deconstruction / demolition X The comparison of construction products must be done with the same function,
applying the same unit declared and at the level of the building (or architectural or
C2 Transport X
Fin de vida engineering work), that is, including the behaviour of the product throughout its
C3 Waste treatment X
life cycle, as well as the specifications of section 6.7.2 of the UNE-EN ISO 14025
C4 Elimination X Standard.
Potential of reuse, recovery
D X
and/or recycling 1.4. Differences when comparing with previous versions
of the present EPD
X = Module included in the LCA; NR = Not relevant module; MNE = Module not evaluated There are no versions prior to the present EPD.
6
HHoott--rroolllleedd rriibbbbeedd sstteeeell pprroocceeeeddiinngg ffrroomm aann eelleeccttrriicc aarrcc ffuurrnnaaccee
2
THE PRODUCT
2.1. Product identification
The EPD is applicable to hot-rolled ribbed steel for construction, produced in an elec-
tric arc furnace.
The MEGASA Group elaborates high ductility steel and special ductility steel, the latter
being designed specifically for structures subject to seismic forces, providing greater
security against brittle fractures.
Ribbed steel, together with concrete, constitutes reinforced concrete, which is one of
the most used constructive elements in the sector.
This product is supplied in diameters from 6mm up to the possibility of 40mm, in diffe-
rent presentations (bar, coil, spooled coil or spool).
CPC code: 4214 - Bars and rods, hot-rolled, of iron or steel.
2.2. Product composition
The manufacturer declares the following composition:
Product composition % in weight
Post-consumer scrap 81 - 82 %
During the product life cycle, no hazardous substances of the “Candidate List of
Pre-consumer scrap 18 – 19 % Substances of Very High Concern (SVHC) for authorisation” was used in a percentage
greater than 0.1% of the product weight.
7
Hot-rolled ribbed steel proceeding from an electric arc furnace
2.3. Product characteristics The chemical composition and remaining characteristics have been established in the
different product Standards of application:
Standards - Ribbed steel Standards - Ribbed steel
UNE 36068 W ree inld foa rb cl ee cr oib nb ce rd et s eteel bars for structural use meant to SS 212540 P for ro cd eu mct es n s tp oe fc cifi oc na ct ri eo tn e f –o r W S eS l- dE aN b l1 e0 r0 e8 in0 fo:2 r0 ci0 ng5 - st S et ee lel for rein-
Weldable ribbed steel bars with special ductility
UNE 36065 Steel for reinforcement of concrete – Dimensions and proper-
characteristics for reinforcement of concrete NS 3576-2
ties – Part 2: Ribbed steel B500NB
Steel for reinforcement of concrete. Weldable reinforcing
BS 4449:2005 steel. Bar, coil and decoiled product. Specification Steel for reinforcement of concrete – Dimensions and proper-
NS 3576-3 ties – Part 2: Ribbed steel B500NC
Steel for reinforcement of concrete. Weldable reinforcing
EN 10080
steel. General
Reinforcing steel. Minimum requirements for weldable reinfor-
SFS 1300
cing steel and welded fabrics
EN 1992-1-1 Eurocode 2 part 3.2 and appendix C
NBN A 24-30 Siderurgique produts. Steel for reinforcement
DIN 488 Reinforcing steel – Reinforcing steel bars.
Steel for reinforcement of concrete. Weldable reinforcing
Steel for reinforcement of concrete - Weldable steels - Part PN-H-93220
NF A35-080 steel B500SP - Ribbed bars and wires
1: bars and coils
Steel products - Reinforcing steel for concrete - Weldable bars
LNEC E449 Steel bars A400NR for reinforcement of concrete NM 01.4.097 and coils with bonding action [MORROCO]
LNEC E450 Steel bars A500NR for reinforcement of concrete G30.18-90 Carbon Steel bars for concrete reinforcement
Steel bars A400NR with special ductility for reinforcement of
LNEC E455 NMX-B-506- Steel industry - Ribbed steel wire for reinforcement of concre-
concrete
CANACERO te - test specifications and methods
Steel bars A500NR with special ductility for reinforcement of
LNEC E460
concrete NMX-B-A457- Steel industry - Low-alloy ribbed steel wire for reinforcement
CANACERO of concrete - test specifications and methods
Standard specification for deformed and plain Carbon-Steel
ASTM A615/615M
bars for concrete reinforcement
Concrete. Carbon steel bar, ribbed or plain, for reinforcement
NTP 341.031
of concrete. Specifications [PERU]
Standard specification for deformed and plain Low-Alloy
ASTM A706/706M
Steel bars for concrete reinforcement
AS/NZS 4671 Steel for reinforcement of concrete
BRL0501 + NEN 6008 Steel for reinforcement of concrete
8
Hot-rolled ribbed steel proceeding from an electric arc furnace
3
INFORMATION RELATIVE TO LCA
3.1. Life cycle assessment
The Report of life cycle assessment for the EPD relative to the steel products of MEGASA
GROUP, dated July 2023, was elaborated by the company Abaleo S.L. with the databases
Ecoinvent 3.9 (January 2023) and Environmental Footprint 3.1 and the SimaPro 9.5.0.0
software, which is the most updated version available when the LCA was prepared.
Electricity, Gas,
To prepare the study, the data from the plants in Spain (Narón and Zaragoza) and Portu- Water, Oxygen, etc. Melt shop
gal (Maia and Seixal) have been taken into account.
The LCA study followed both the recommendations and requirements of the international
ISO 14040:2006, ISO 14044:2006, UNE 36904-1:2018 and UNE-EN 15804:2012+A2:2019
Standards.
3.2. Scope of the study Scrap and others
ferrous materials
The scope of the EPD is the cradle-to-door production with options (modules A1-A3, A4, C
Rolling mill
and D) of the ribbed steel elaborated by the MEGASA GROUP for use as structural systems
in the construction sector.
The specific data of the manufacturing process come from the Spanish plants (Narón and
Ferroalloys
Zaragoza) and the Portuguese ones (Maia and Seixal), corresponding to the year 2022. and other additives
The LCA does not include the following:
All equipment with a service life superior to 3 years.
The construction of plant buildings; other capital goods.
Consumables: Rebar Steel in
Staff work travel; the staff’s travel to or from work.
electrodes, refractories, bars and coils
Research and development activities. etc...
9
HHoott--rroolllleedd rriibbbbeedd sstteeeell pprroocceeeeddiinngg ffrroomm aann eelleeccttrriicc aarrcc ffuurrnnaaccee
3.3. Declared unit
The declared unit is one tonne of product, including its
distribution packaging.
3.4. Allocation criteria
According to the criteria of the reference standard:
Where possible, the product system has been extended to avoid the allocation of
environmental impacts of co-products.
When it was not possible to avoid the allocation, an allocation of the inputs and
outputs of the system has been made (based on mass).
It has not been necessary to apply economic allocation criteria.
3.5. Cut-off rule
In accordance with the criteria of the reference standard, the gross weight/volume of
all materials used in the manufacturing process has been included in the LCA, so that at
least 99% of the weight of the product unit is obtained.
There has been no exclusion of either material or energy consumption.
1100
Hot-rolled ribbed steel proceeding from an electric arc furnace
3.6. Representativeness, quality and selection of data Very good integrity. Score 1.
Good methodological suitability and coherence. Score 2.
To model the steel manufacturing process of the MEGASA GROUP’s ribbed steel, the Very good temporal representativeness. Score 1.
factories’ production data for the year 2022 have been used, which is a period con- Very good technological representativeness. Score 1.
sidered representative of an average production. From these factories, the following Very good geographical representativeness. Score 1.
data have been obtained: consumption of material and energy; emissions to air and Very low data uncertainty. Score 1.
discharges to water; distances from suppliers; waste generation and waste manage-
ment. According to the previous data, the Data Quality Rating (DQR) takes the following
value: 7/6 = 1.17, which indicates that the quality of the data is excellent.
When necessary, the Ecoinvent 3.9 (January 2023) and Environmental Footprint 3.1
databases have been used, which are the latest versions available at the time of the To better understand the data quality assessment carried out, it is indicated that the
LCA. For the inventory data, the most up-to-date version of SimaPro 9.5.0.0 softwa- score of each of the criteria varies from 1 to 5 (the lower the score, the more quality)
re available at the time of the study has been used to model the LCA and to calculate and that the following table is applied to obtain the final score:
the environmental impact categories requested by the reference standard.
For the selection of the most representative processes, the following criteria have
Overall Data Quality Rating
been applied: Overall data quality level
(DQR)
≤ 1.6 Excellent quality
They had to be representative data of the technological development actually
applied in the manufacturing processes. If case of no information available,
representative data of an average technology have been chosen. 1.6 a 2.0 Very good quality
They had to be geographical data as close as possible and, where appropriate,
regionalized means.
2.0 a 3.0 Good quality
They had to be the most current data possible.
3 a 4.0 Reasonable quality
To assess the quality of the primary data of the production for the product under
study, the criteria of semi-quantitative evaluation of the data quality proposed by the
European Union in its Guide to the Environmental Footprint of Products and Organi- > 4 Insufficient quality
sations are applied. The results obtained are as follows:
11
Hot-rolled ribbed steel proceeding from an electric arc furnace
4
LIMITS TO THE SYSTEM,
SCENARIOS AND ADDITIONAL
The product system studied in the Life Cycle Assessment of the ribbed steel produ-
TECHNICAL INFORMATION
ced by the MEGASA GROUP is cradle-to-door with options. The following steps of
production were studied:
Module A1: Production of raw materials
This module includes the production process of raw materials,
which considers:
Extraction of resources and production of raw materials.
Transport to the processing/production centres of raw materials.
Energy and fuel consumption during the production of raw materials.
The consumption of other resources (such as water), during the production
of raw materials.
The generation of waste and emissions to the air and discharges to water and
soil, during the production of raw materials.
The production of the electricity used in the manufacturing process.
The scrap enters the plant as a residue, where it is processed as a secondary
raw material.
Module A2: Transport
The transport by lorry, ship and train of all raw materials has been considered from
the production sites (suppliers) to the Megasa Group’s plants in Spain (Narón and Za-
ragoza) and Portugal (Maia and Seixal). The transport distances of the raw materials
have been calculated based on the locations showing in the databases of the purcha-
sing and sales departments. Scrap enters the plant as waste, so its transport corres-
ponds to the previous product system.
12
HHoott--rroolllleedd rriibbbbeedd sstteeeell pprroocceeeeddiinngg ffrroomm aann eelleeccttrriicc aarrcc ffuurrnnaaccee
Module A3: Manufacturing
At this stage, the consumption of auxiliary materials in the production (auxiliary
materials and general plant consumption) has been considered; the production of the
necessary packaging to distribute the product to customers and its transport to the
plant; emissions to air and water, as well as transport to the manager of the waste
generated during this stage of the life cycle. The following co-products are generated
in the production process: black slag and mill scale
The transport distances of the waste have been calculated based on the locations
showing in the databases of the purchasing and sales departments.
Module A4: Transport to the place of use
The transport of the finished product from the plants where the steel is made up to
the customer has been considered, with data from the year 2022, distinguishing the
means of transport used: lorry, ship or train.
Quantity
Parameter
(per unit declared)
Lorry EURO 5 (max. weight
0.0451 l/tkm
authori. 15.79 t)
Litres of diesel
Ship 0.0026 l/tkm
Train 0.0129 l/tkm
Lorry EURO 5 710.63 km
Average distance Ship 2146.61 km
Train 357.61 km
Load factor (including empty return) 50%
Bulk density of products transported -
Useful capacity factor -
13
Hot-rolled ribbed steel proceeding from an electric arc furnace
Module C1 – Deconstruction / demolition.
Parameter Value (per unit declared)
For the LCA it has been taken into account that the deconstruction modulus (C1) is not
The consumption of material and
considered relevant for quantitative analysis. The consumption of material and ener-
energy for the deconstruction and
gy for the deconstruction and extraction of the MEGASA GROUP’s steel products are
extraction of the Megasa Group’s
included in the framework of the building or civil works of which they form part. Demolition steel products are included in the fra-
mework of the building or civil works of
which they form part.
Module C2: Transport to the place of waste treatment/
0 kg for reuse.
recovery
Recovery system,
1000 kg for recycling.
It is considered that, at the end of its useful life, the product under study is transported specified by type
to the point of waste management by road, ship or train. The average transport of
0 kg for energy recovery.
the scrap received by the MEGASA GROUP’s plants, authorized as a waste treatment
facility for recovery operations (R4 – recycling or recovery of metals and metal com-
Elimination, specified by type 0 kg for final disposal (landfill):
pounds), has been considered.
Lorry EURO 5:
106.18 km
Module C3 - Waste treatment,
and Module C4 - Waste elimination Transport of
Assumptions for scenario
waste up to Ship: 1598.59 km
development (transport)
manager:
The waste scenario considered establishes that the products under study are sent to
recycling for the recovery of steel as a secondary material. Train: 349.23 km
Module D – Charges and benefits beyond the limit
of the system
Module D includes the potential for reuse and recycling expressed as net charges and
benefits relative to secondary material recovered when leaving the product system,
calculating material substitution effects only for the resulting net output stream from
the product stage; the secondary material used as input in the product stage (A1-A3)
has been excluded, considering only the % of non-secondary raw material that rea-
ches the waste conditions.
14
Hot-rolled ribbed steel proceeding from an electric arc furnace
Product stage
A1 A2 A3
X X X
15
slairetam
war
fo
ylppuS
tropsnarT
gnirutcafunaM
A1 a A3
Stage of use
B1 B2 B3 B4 B5 B6 B7
MNE MNE MNE MNE MNE MNE MNE
esU
ecnanetniaM
gniriapeR
tnemecalpeR noitatilibaheR
ecivres
ni
esu
ygrenE
ecivres
ni
esu
retaW
B1 a B7
End-of-life stage
C1 C2 C3 C4
X X X X
Sce- Sce- Sce- Sce- Sce- Sce- Sce-
nario nario nario nario nario nario nario
noitilomed
,noitcurtsnoceD
tropsnarT
tnemtaert
etsaW
noitanimile
etsaW
C1 a C4
Stage of
construction
process
A4 A5
X MNE
Sce- Sce- Sce- Sce-
nario nario nario nario
tropsnarT
noitallatsni
/ noitcurtsnoC
ssecorp
A4 a A5
Charges and be-
nefits beyond the
limit of the system
D
X
Sce- Sce-
nario nario
yrevocer
,esuer
fo
laitnetoP
gnilcycer
ro/dna
Additional
Life cycle assessment. - UNE EN 15804
information
D
X: Módulo evaluado. / MNE: Módulo no evaluado.
Hot-rolled ribbed steel proceeding from an electric arc furnace
5
DECLARATION OF THE ENVIRONMENTAL PARAMETERS OF LCA AND LCI
Environmental impact parameters for 1 tonne of ribbed steel
Environmental impact parameters defined in the UNE-EN 15804 Standard
Ribbed steel. Unit declared: 1 tonne
Parameter Unit A1 A2 A3 A1-A3 A4 C1 C2 C3 C4 D
GWP-total kg CO2 eq 2.31E+02 7.45E+00 8.57E+01 3.24E+02 4.60E+01 0.00E+00 4.45E+01 0.00E+00 0.00E+00 0.00E+00
GWP-fossil kg CO2 eq 2.27E+02 7.45E+00 8.56E+01 3.20E+02 4.60E+01 0.00E+00 4.45E+01 0.00E+00 0.00E+00 0.00E+00
GWP-biogenic kg CO2 eq 3.19E+00 4.26E-04 1.00E-01 3.29E+00 2.60E-03 0.00E+00 2.36E-03 0.00E+00 0.00E+00 0.00E+00
GWP-luluc kg CO2 eq 7.25E-01 1.65E-04 1.60E-02 7.41E-01 1.05E-03 0.00E+00 1.34E-03 0,00E+00 0.00E+00 0.00E+00
ODP kg CFC-11 eq 1.01E-05 1.52E-07 7.03E-07 1.09E-05 9.22E-07 0.00E+00 7.72E-07 0.00E+00 0.00E+00 0.00E+00
AP mol H+ eq 8.00E-01 5.81E-02 7.21E-02 9.31E-01 4.39E-01 0.00E+00 6.79E-01 0.00E+00 0.00E+00 0.00E+00
EP-freshwater kg P eq 4.74E-03 5.76E-06 3.76E-04 5.12E-03 3.54E-05 0.00E+00 3.20E-05 0.00E+00 0.00E+00 0.00E+00
EP-marine kg N eq 1.50E-01 1.68E-02 6.65E-02 2.33E-01 1.28E-01 0.00E+00 2.10E-01 0.00E+00 0.00E+00 0.00E+00
EP-terrestrial mol N eq 1.68E+00 1.83E-01 2.94E-01 .16E+00 1.40E+00 0.00E+00 2.31E+00 0,00E+00 0.00E+00 0.00E+00
POFP kg NMVOC eq 8.10E-01 5.67E-02 2.15E-01 1.08E+00 4.17E-01 0.00E+00 6.45E-01 0.00E+00 0.00E+00 0.00E+00
ADP-minerals&-
kg Sb eq 4.46E-05 2.26E-07 1.36E-05 5.84E-05 1.34E-06 0.00E+00 1.17E-06 0.00E+00 0.00E+00 0.00E+00
metals 2
ADP-fossil 2 MJ, v.c.n. 4.30E+03 9.72E+01 2.11E+02 4.61E+03 5.97E+02 0.00E+00 5.71E+02 0.00E+00 0.00E+00 0.00E+00
WDP 2 m3 eq 1.21E+02 8.80E-02 6.07E+01 1.82E+02 5.37E-01 0.00E+00 5.00E-01 0.00E+00 0.00E+00 0.00E+00
16
HHoott--rroolllleedd rriibbbbeedd sstteeeell pprroocceeeeddiinngg ffrroomm aann eelleeccttrriicc aarrcc ffuurrnnaaccee
GWP-total. Global warming potential.
GWP-fossil. Global warming potential of fossil fuels.
GWP-biogenic. Biogenic global warming potential.
GWP-luluc. Global warming potential of land use and land-use changes.
ODP. Stratospheric ozone depletion potential.
AP. Acidification potential, accumulated surplus.
EP-freshwater. Eutrophication potential, fraction of nutrients reaching the
final freshwater compartment.
EP-marine. Eutrophication potential, fraction of nutrients reaching the
final seawater compartment.
EP-terrestrial. Eutrophication potential, accumulated surplus.
POFP. Potential for formation of photochemical oxidants.
ADP-minerals&metals. Abiotic resource depletion potential for
non-fossil resources.
APD-fossil. Abiotic resource depletion potential for fossil resources.
WDP. Water deprivation potential (user), water weighted deprivation
consumption.
1177
Hot-rolled ribbed steel proceeding from an electric arc furnace
Additional parameters of environmental impact defined in the UNE-EN 15804 Standard
Ribbed steel. Unit declared: 1 tonne
Parameter Unit A1 A2 A3 A1-A3 A4 C1 C2 C3 C4 D
Incidence of
PM 1.46E-05 4.40E-07 2.08E-06 1.72E-05 2.72E-06 0.00E+00 3.09E-06 0.00E+00 0.00E+00 0.00E+00
diseases
IRP ¹ kBq U235 eq 3.46E+01 1.47E-02 4.01E-01 3.50E+01 8.91E-02 0.00E+00 7.21E-02 0.00E+00 0.00E+00 0.00E+00
ETP-fw ² CTUe 6.29E+02 4.39E+01 2.45E+02 9.17E+02 2.74E+02 0.00E+00 2.89E+02 0.00E+00 0.00E+00 0.00E+00
HTP-c ² CTUh 1.31E-06 6.22E-10 6.36E-07 1.94E-06 3.93E-09 0.00E+00 3.83E-09 0.00E+00 0.00E+00 0.00E+00
HTP-nc ² CTUh 9.74E-07 4.64E-08 5.20E-06 6.22E-06 2.64E-07 0.00E+00 1.70E-07 0.00E+00 0.00E+00 0.00E+00
SQP ² Pt 1.06E+03 1.77E-01 7.93E+02 1.85E+03 1.07E+00 0.00E+00 8.94E-01 0.00E+00 0.00E+00 0.00E+00
PM. Potential incidence of diseases due to emissions of particulate Note 1
matter.
This impact category deals primarily with the eventual impacts of low doses of
IRP. Human potential exposure efficiency relative to U235. ionizing radiation on human health from the nuclear fuel cycle. It does not consider
effects due to possible nuclear accidents or occupational exposure due to the dispo-
ETP-fw. Comparative potential of toxic unit for ecosystems - sal of radioactive waste in underground facilities. The potential for ionizing radiation
freshwater.
of the soil, due to radon or building materials, is not measured in this parameter
either
HTP-c. Comparative potential of toxic unit for ecosystems -
carcinogenic effects.
Note 2
HTP-nc. Comparative potential of toxic unit for ecosystems -
non-carcinogenic effects. The results of this environmental impact indicator should be used with caution as the
uncertainties of the results are high and experience with this parameter is limited.
SQP. Soil quality potential index.
18
Hot-rolled ribbed steel proceeding from an electric arc furnace
Use of resources for 1 tonne of ribbed steel
Ribbed steel. Unit declared: 1 tonne
Parameter Unit A1 A2 A3 A1-A3 A4 C1 C2 C3 C4 D
PERE MJ, v.c.n. 7.33E+02 2.41E-01 1.04E+01 7.44E+02 1.45E+00 0.00E+00 1.14E+00 0.00E+00 0.00E+00 0.00E+00
PERM MJ, v.c.n. 0.00E+00 0.00E+00 0.00E+00 0.00E+00 0.00E+00 0.00E+00 0.00E+00 0.00E+00 0.00E+00 0.00E+00
PERT MJ, v.c.n. 7.33E+02 2.41E-01 1.04E+01 7.44E+02 1.45E+00 0.00E+00 1.14E+00 0.00E+00 0.00E+00 0.00E+00
PENRM MJ, v.c.n. 5.41E-02 3.82E-05 5.11E+01 5.11E+01 2.80E-04 0,00E+00 9.06E-04 0.00E+00 0.00E+00 0.00E+00
PENRE MJ, v.c.n. 5.73E+03 9.77E+01 2.26E+02 6.05E+03 6.00E+02 0.00E+00 5.73E+02 0.00E+00 0.00E+00 0.00E+00
PENRT MJ, v.c.n. 5.73E+03 9,77E+01 2.77E+02 6.10E+03 6.00E+02 0.00E+00 5.73E+02 0.00E+00 0.00E+00 0.00E+00
SM kg 1.14E+03 0.00E+00 0.00E+00 1.14E+03 0.00E+00 0.00E+00 0.00E+00 0.00E+00 0.00E+00 0.00E+00
RSF MJ, v.c.n. 0.00E+00 0.00E+00 0.00E+00 0.00E+00 0.00E+00 0.00E+00 0.00E+00 0.00E+00 0.00E+00 0.00E+00
NRSF MJ, v.c.n. 0.00E+00 0.00E+00 0.00E+00 0.00E+00 0.00E+00 0.00E+00 0.00E+00 0.00E+00 0.00E+00 0.00E+00
FW m3 2.78E+00 4.03E-03 1.34E+00 4.12E+00 2.46E-02 0.00E+00 2.24E-02 0.00E+00 0.00E+00 0.00E+00
PERE. Use of renewable primary energy excluding renewable primary PENRT. Total use of non-renewable primary energy.
energy resources used as raw material.
SM. Use of secondary materials.
PERM. Use of renewable primary energy used as raw material.
RSF. Use of renewable secondary fuels.
PERT. Total use of renewable primary energy.
NRSF. Use of non-renewable secondary fuels.
PENRE. Use of non-renewable primary energy, excluding non-renewa-
ble primary energy resources used as raw material.
FW. Net use of running water resources.
PENRM. Use of non-renewable primary energy used as raw material.
19
Hot-rolled ribbed steel proceeding from an electric arc furnace
Categories of wastes for 1 tonne of ribbed steel
Parameters describing the generation of residue.
Ribbed steel. Unit declared: 1 tonne
Parameter Unit A1 A2 A3 A1-A3 A4 C1 C2 C3 C4 D
HWD kg 1.71E-02 6.14E-04 1.16E-03 1.89E-02 3.72E-03 0.00E+00 3.45E-03 0.00E+00 0.00E+00 0.00E+00
NHWD kg 2.40E+01 5.00E-03 9.96E+00 3.40E+01 3.09E-02 0.00E+00 3.22E-02 0.00E+00 0.00E+00 0.00E+00
RWD kg 2.07E-02 7.65E-06 2.64E-04 2.10E-02 4.58E-05 0,00E+00 3.25E-05 0.00E+00 0.00E+00 0.00E+00
HWD. Hazardous wastes eliminated. NHWD. Non-hazardous wastes eliminated. HWD. Radioactive wastes eliminated.
Output flows for 1 tonne of ribbed steel
Parameters describing the output flows.
Ribbed steel. Unit declared: 1 tonne
Parameter Unit A1 A2 A3 A1-A3 A4 C1 C2 C3 C4 D
CRU kg 0.00E+00 0.00E+00 1.33E+02 1.33E+02 0.00E+00 0.00E+00 0.00E+00 0.00E+00 0.00E+00 0.00E+00
MFR kg 0.00E+00 0.00E+00 4.03E+01 4.03E+01 0.00E+00 0.00E+00 0.00E+00 1.00E+00 0.00E+00 0.00E+00
MER kg 0.00E+00 0.00E+00 1.99E-01 1.99E-01 0.00E+00 0.00E+00 0.00E+00 0.00E+00 0.00E+00 0.00E+00
EE MJ 0.00E+00 0.00E+00 0.00E+00 0.00E+00 0.00E+00 0.00E+00 0.00E+00 0.00E+00 0.00E+00 0.00E+00
CRU. Components for their reuse. MFR. Materials for recycling. MER. Materials for energy valuation EE. Exported energy.
20
Hot-rolled ribbed steel proceeding from an electric arc furnace
6
INFORMACIÓN
AMBIENTAL ADICIONAL
6.1. Emissions to indoor air
The manufacturer declares that the steel products under study do not generate emis-
sions to indoor air during their useful life.
6.2. Emissions to soil and water
The manufacturer declares that the steel products under study do not generate emis-
sions either to soil or to water during their useful life.
6.3. Biogenic carbon content
The manufacturer declares that the steel products under study do not include mate-
rials with biological content.
The packaging with biogenic carbon used to distribute MEGASA’s product is less than
1% of the weight of the product. Following the indications of the reference standard,
the declaration of the biogenic carbon content of the packaging is omitted because
the mass of the materials containing biogenic carbon in the packaging is less than 5%
of the total mass of the product.
21
Hot-rolled ribbed steel proceeding from an electric arc furnace
7
REFERENCES
UNE-EN 36904-1 Standard. Iron and Steel industry. Environmental Product UNE-EN ISO 14040:2006/A1:2021. Environmental Management. Life cycle assessment.
Declarations. Product Category Rules. Steel products for structures. Part 1: Basic Principles and reference framework. Modification 1. (ISO 14040:2006/Amd 1:2020).
products. 2018.
UNE-EN ISO 14044:2006/A1:2021 Standard. Environmental Management. Life cycle as-
UNE-EN 15804:2012+A2:2019. Sustainability in construction. Environmental Product sessment. Requirements and guidelines. Modification 2. (ISO 14044:2006/Amd 2:2020).
Declarations. Basic product-category rules for construction products.
Report of life cycle assessment for the EPDs relative to the MEGASA GROUP’s steel pro-
General rules of the GlobalEPD program, 2nd revision. AENOR. February 2016. ducts. Drafted by Abaleo S.L, August 2023. Version 2..
UNE-EN ISO 14025:2010 Environmental labels. Environmental Declarations, type III. Databases: Ecoinvent 3.9.1 (January 2023) and Environmental Footprint 3.1.
Principles and procedures (ISO 14025:2006).
Environmental impact assessment methodologies implemented through SimaPro 9.5.0.0
2222
Hot-rolled ribbed steel proceeding from an electric arc furnace
Environmental Product Declaration
23
