Environmental product declaration
in accordance with ISO 14025 and EN 15804+A2
Housegard 6 kg Powder Extinguisher, PE6HR-A, 55A 233B C
Owner of the declaration: Program operator:
GPBM Nordic AB The Norwegian EPD Foundation
Product: Declaration number:
Housegard 6 kg Powder Extinguisher, PE6HR-A, 55A
233B C NEPD-9388-8982
Declared unit: Registration number:
1 pcs
NEPD-9388-8982
This declaration is based on Product Category Rules:
Issue date: 14.03.2025
CEN Standard EN 15804:2012+A2:2019 serves as core
The Norwegian EPD Foundation PCR Valid to: 14.03.2030
PCR 2010:08 for other special- and general-purpose
machinery and parts thereof., ver. 4.0, 04.04.2022. The EPD software:
International EPD® System. LCAno EPD generator ID: 755519
1 / 12
General information
Product Owner of the declaration:
Housegard 6 kg Powder Extinguisher, PE6HR-A, 55A 233B C GPBM Nordic AB
Contact person: Malin Strelitzsky
Phone: +46(0)31-7991600
e-mail: info@gpbmnordic.se
Program operator: Manufacturer:
The Norwegian EPD Foundation GPBM Nordic AB
Post Box 5250 Majorstuen, 0303 Oslo, Norway Sörredsvägen 113
Phone: +47 977 22 020 41878 Göteborg, Sweden
web: www.epd-norge.no
Declaration number: Place of production:
GPBM Nordic AB - Production site China
NEPD-9388-8982
, China
This declaration is based on Product Category Rules: Management system:
CEN Standard EN 15804:2012+A2:2019 serves as core PCR
PCR 2010:08 for other special- and general-purpose machinery and
parts thereof., ver. 4.0, 04.04.2022. The International EPD® System.
Statement of liability: Organisation no:
The owner of the declaration shall be liable for the underlying 556360-0443
information and evidence. EPD Norway shall not be liable with respect
to manufacturer information, life cycle assessment data and
evidences.​
Declared unit: Issue date:
1 pcs Housegard 6 kg Powder Extinguisher, PE6HR-A, 55A 233B C
14.03.2025
Declared unit with option: Valid to:
A1-A3,A4,A5,B2,B6,C1,C2,C3,C4,D
14.03.2030
Year of study:
2023
Functional unit: Comparability:
Not applicable. EPD of construction products may not be comparable if they do not
comply with EN 15804 and seen in a building context.
General information on verification of EPD from EPD tools: Development and verification of EPD:
Independent verification of data, other environmental information The declaration is created using EPD tool lca.tools ver EPD2022.03,
and the declaration according to ISO 14025:2010, § 8.1.3 and § 8.1.4. developed by LCA.no. The EPD tool is integrated in the company's
Verification of each EPD is made according to EPD-Norway’s management system, and has been approved by EPD Norway.
guidelines for verification and approval requiring that tools are i) NEPDT151
integrated into the company's environmental management system, ii)
the procedures for use of the EPD tool are approved by EPD-Norway, Developer of EPD: Malin Strelitzsky
​
and iii) the process is reviewed annually by an independent third
Reviewer of company-specific input data and EPD: Merja Pulkkinen
party verifier. See Appendix G of EPD-Norway's General Programme
Instructions for further information on EPD tools
Verification of EPD tool:
Independent third party verification of the EPD tool, background data Approved:
and test-EPD in accordance with EPDNorway's procedures and
guidelines for verification and approval of EPD tools.
Third party verifier:
Elisabet Amat, GREENIZE projects
(no signature required)
2 / 12
Product
Product description:
6kg ABC Powder Fire extinguisher.
The product is suitable for residential, office, industrial, and automotive use.
Product specification
The product is made with 11% recycled steel
Materials kg %
Ethylene propylene diene monomer
0,11 1,25
(EPDM)
Metal - Steel low alloy 2,72 29,52
Plastic - Polyamide 0,0088 0,095
Plastic - Polytetrafluoroethylene
0,00017 0,0018
(PTFE)
Polyvinyl chloride (PVC) 0,055 0,59
Metal - Aluminium alloy 0,28 3,11
Metal - Brass 0,033 0,35
Chemical 6.00 65,054
Total 9,22 100,00
Packaging kg %
Packaging - Cardboard 0,40 97,32
Packaging - Paper 0,01 2,68
Total incl. packaging 9,63 100,00
Technical data:
Standard: EN 3-7
Certifications: CE, Wheelmark
Technical data
Fire class ABC
Efficiency class 55A 233B C
Temperature range -30 °C / +60 °C
Extinguishing agent SUN ABC PWR
Extinguisher size 6 kg
Discharge time 23 s
Throwing range 4-6 m
Working pressure 15 bar
Cylinder material Steel
Propellant Nitrogen
Height 520 mm
Width 150 mm
Market:
Nordic
Reference service life, product
10 years
Reference service life, building or construction works
N/A
LCA: Calculation rules
Declared unit:
1 pcs Housegard 6 kg Powder Extinguisher, PE6HR-A, 55A 233B C
Cut-off criteria:
All major raw materials and all the essential energy is included. The production processes for raw materials and energy flows with very small
amounts (less than 1%) are not included. These cut-off criteria do not​ apply for hazardous materials and substances.
Allocation:
The allocation is made in accordance with the provisions of EN 15804. Incoming energy and water and waste production in-house is allocated
equally among all products through mass allocation. Effects of primary production of recycled materials is allocated to the main product in which
the material was used. The recycling process and transportation of the material is allocated to this analysis.
Data quality:
3 / 12
Specific data for the product composition are provided by the manufacturer. The data represent the production of the declared product and were
collected for EPD development in the year of study. Background data is based on EPDs according to EN 15804 and different LCA databases. The
data quality of the raw materials in A1 is presented in the table below.
Materials Source Data quality Year
Chemical ecoinvent 3.10 Database 2023
Ethylene propylene diene monomer (EPDM) ecoinvent 3.6 Database 2019
Metal - Aluminium alloy ecoinvent 3.6 Database 2019
Metal - Brass ecoinvent 3.6 Database 2019
Metal - Steel low alloy ecoinvent 3.6 Database 2019
Packaging - Cardboard Modified ecoinvent 3.6 Database 2019
Packaging - Paper ecoinvent 3.6 Database 2019
Plastic - Polyamide ecoinvent 3.6 Database 2019
Plastic - Polytetrafluoroethylene (PTFE) ecoinvent 3.6 Database 2019
Polyvinyl chloride (PVC) ecoinvent 3.6 Database 2019
4 / 12
System boundaries (X=included, MND=module not declared, MNR=module not relevant)
Construction Beyond the system
Product stage Use stage End of life stage
installation stage boundaries
A1 A2 A3 A4 A5 B1 B2 B3 B4 B5 B6 B7 C1 C2 C3 C4 D
X X X X X MND X MND MND MND X MND X X X X X
System boundary:
This EPD includes A1-D.
B1 - B7 are not relevant.
Modules A1-A4 are included in the analysis. It includes the extraction and production of raw materials, transportation to the factory, the
production process itself and transportation to market.
Additional technical information:
Maintenance of fire extinguishers shall be carried out in accordance with national standards and the manufacturer's service instructions.
waR slairetam tropsnarT gnirutcafunaM tropsnarT ylbmessA e​sU ecnanetniaM riapeR tnemecalpeR tnemhsibrufeR lanoitarepO ygrene esu lanoitarepO esu retaw -eD noitcurtsnoc noitilomed tropsnarT etsaW gnissecorp lasopsiD -yrevoceR-esueR laitnetop-gnilcyceR
5 / 12
LCA: Scenarios and additional technical information
The following information describe the scenarios in the different modules of the EPD.
All materials are reused or recycled at end of life.
Module A4: transport includes the import from China to Sweden and distribution into the nordic market.
Module B2 is declared as zero because the general maintenance only includes visual inspection of the pressure.
Module B6 is declared as zero because there is no operational energy usage.
Module C1 is declared as zero because it is assumed that the disassembly of fire extinguishers are done manually.
Capacity utilisation Value
Transport from production place to user (A4) Distance (km) Fuel/Energy Consumption Unit
(incl. return) % (Liter/tonne)
Ship, Freight, Transoceanic (km) 65,0 % 22000 0,003 l/tkm 66,00
Truck, 16-32 tonnes, EURO 4 (km) - Europe 36,7 % 5 0,044 l/tkm 0,22
Truck, 16-32 tonnes, EURO 4 (km) - Europe 36,7 % 1000 0,044 l/tkm 44,00
Truck, 16-32 tonnes, EURO 4 (km) - World 38,8 % 100 0,045 l/tkm 4,50
Assembly (A5) Unit Value
Waste, packaging, corrugated board box, 0 %
kg 0,40
recycled, to average treatment (kg)
Waste, packaging, paper printed, to average
kg 0,011
treatment (kg)
Capacity utilisation Value
Transport to waste processing (C2) Distance (km) Fuel/Energy Consumption Unit
(incl. return) % (Liter/tonne)
Truck, 16-32 tonnes, EURO 6 (km) - Europe 36,7 % 85 0,043 l/tkm 3,66
Waste processing (C3) Unit Value
Steel to recycling (kg) kg 2,72
Aluminium to recycling (kg) kg 0,28
Plastics to recycling (kg) kg 0,17
Brass to recycling (kg) kg 0,033
Waste treatment per kg Plastic, Mixture,
kg 0,00017
municipal incineration with fly ash extraction (kg)
Chemical to recycling (kg) kg 6.00
Disposal (C4) Unit Value
Landfilling of ashes from incineration of Plastics,
Mixture, municipal incineration with fly ash
kg 0,0000059
extraction, process per kg ashes and residues - C4
(kg)
Benefits and loads beyond the system
Unit Value
boundaries (D)
Substitution of primary steel with net scrap (kg) kg 2,42
Substitution of primary aluminium with net scrap
kg 0,24
(kg)
Substitution of Polyvinylchloride, average, PVC
kg 0,055
(kg)
Substitution, ethylene propylene diene monomer
kg 0,11
(EPDM) (kg)
Substitution of primary Brass with net scrap (kg) kg 0,022
Substitution of electricity, in Norway (MJ) MJ 0,023
Substitution of thermal energy, district heating, in
MJ 0,35
Norway (MJ)
Substitution of polyamide, nylon 6, granulate (kg) kg 0,0087
Substitution, monoammonium phosphate (kg) kg 6.00
6 / 12
LCA: Results
The LCA results are presented below for the declared unit defined on page 2 of the EPD document.
Environmental impact
Indicator Unit A1-A3 A4 A5 B2 B6 C1 C2 C3 C4 D
GWP-total
kg CO2 -
2,13E+01 3,76E+00 7,05E-01 0 0 0 1,34E-01 4,02E-04 1,69E-08 -1,20E+01
eq
GWP-fossil
kg CO2 -
2,18E+01 3,76E+00 6,65E-03 0 0 0 1,34E-01 4,02E-04 1,69E-08 -1,19E+01
eq
GWP-biogenic
kg CO2 -
-6,18E-01 1,27E-03 6,98E-01 0 0 0 5,54E-05 8,74E-09 9,00E-12 2,52E-02
eq
GWP-luluc
kg CO2 -
5,07E-02 2,00E-03 2,20E-06 0 0 0 4,76E-05 1,63E-09 2,00E-12 -7,79E-02
eq
kg
ODP CFC11 - 1,59E-06 8,28E-07 1,40E-09 0 0 0 3,03E-08 1,00E-12 0,00E+00 -1,52E-04
eq
mol H+
AP 1,36E-01 7,39E-02 3,15E-05 0 0 0 3,84E-04 8,82E-08 5,40E-11 -7,75E-02
-eq
EP-FreshWater kg P -eq 3,01E-03 2,25E-05 5,46E-08 0 0 0 1,07E-06 7,80E-11 0,00E+00 -2,58E-03
EP-Marine kg N -eq 2,36E-02 1,90E-02 1,04E-05 0 0 0 7,61E-05 4,22E-08 1,60E-11 -1,20E-02
mol N -
EP-Terrestial 2,83E-01 2,11E-01 1,13E-04 0 0 0 8,51E-04 4,32E-07 1,86E-10 -1,52E-01
eq
kg
POCP NMVOC 8,88E-02 5,56E-02 3,24E-05 0 0 0 3,26E-04 1,04E-07 5,10E-11 -4,56E-02
-eq
ADP- kg Sb-
1,28E-03 6,30E-05 1,62E-07 0 0 0 3,69E-06 4,40E-11 0,00E+00 -8,45E-04
minerals&metals1 eq
ADP-fossil1 MJ 2,46E+02 5,23E+01 9,30E-02 0 0 0 2,02E+00 5,53E-05 1,31E-07 -1,44E+02
WDP1 m3 1,49E+02 2,91E+01 1,18E-01 0 0 0 1,96E+00 3,99E-04 1,68E-06 -1,12E+03
GWP-total = Global Warming Potential total; GWP-fossil = Global Warming Potential fossil fuels; GWP-biogenic = Global Warming Potential biogenic; GWP-luluc =
Global Warming Potential land use and land use change; ODP = Depletion potential of the stratospheric ozone layer; AP = Acidification potential, Accumulated
Exceedance; EP-freshwater = Eutrophication potential, fraction of nutrients reaching freshwater end compartment: EP-marine = Eutrophication potential, fraction of
nutrients reaching marine end compartment; EP-terrestrial = Eutrophication potential, Accumulated Exceedance; POCP = Formation potential of tropospheric ozone;
ADP-minerals&metals = Abiotic depletion potential for non-fossil resources; ADP-fossil = Abiotic depletion for fossil resources potential; WDP = Water (user)
deprivation potential, deprivation-weighted water consumption
"Reading example: 9,0 E-03 = 9,0*10-3 = 0,009"
*INA Indicator Not Assessed
1. The results of this environmental impact indicator shall be used with care as the uncertainties on these results are high or as there is limited experienced with the
indicator
Remarks to environmental impacts
Not applicable.
7 / 12
Additional environmental impact indicators
Indicator Unit A1-A3 A4 A5 B2 B6 C1 C2 C3 C4 D
PM Disease incidence 1,53E-06 1,28E-07 4,64E-10 0 0 0 8,19E-09 0,00E+00 0,00E+00 -7,45E-07
IRP2 kgBq U235 -eq 6,16E-01 2,26E-01 3,98E-04 0 0 0 8,84E-03 1,39E-07 6,48E-10 -4,49E-01
ETP-fw1 CTUe 7,51E+02 3,47E+01 1,24E-01 0 0 0 1,50E+00 8,50E-04 2,88E-07 -3,07E+02
HTP-c1 CTUh 1,01E-07 0,00E+00 4,00E-12 0 0 0 0,00E+00 0,00E+00 0,00E+00 -3,93E-08
HTP-nc1 CTUh 7,17E-07 2,13E-08 1,57E-10 0 0 0 1,64E-09 1,00E-12 0,00E+00 2,96E-08
SQP1 dimensionless 1,56E+02 2,19E+01 6,24E-02 0 0 0 1,41E+00 1,01E-05 3,90E-07 -4,42E+01
PM = Particulate Matter emissions; IRP = Ionizing radiation – human health; ETP-fw = Eco toxicity – freshwater; HTP-c = Human toxicity – cancer effects; HTP-nc =
Human toxicity – non cancer effects; SQP = Potential Soil Quality Index (dimensionless)
"Reading example: 9,0 E-03 = 9,0*10-3 = 0,009"
*INA Indicator Not Assessed
1. The results of this environmental impact indicator shall be used with care as the uncertainties on these results are high or as there is limited experienced with the
indicator
2. This impact category deals mainly with the eventual impact of low dose ionizing radiation on human health of the nuclear fuel cycle. It does not consider effects due
to possible nuclear accidents, occupational exposure nor due to radioactive waste disposal in underground facilities. Potential ionizing radiation from the soil, from
radon and from some construction materials is also not measured by this indicator.
8 / 12
Resource use
Indicator Unit A1-A3 A4 A5 B2 B6 C1 C2 C3 C4 D
PERE MJ 3,28E+01 5,43E-01 1,53E-03 0 0 0 2,90E-02 3,08E-06 9,14E-09 -1,90E+01
PERM MJ 6,52E+00 0,00E+00 -6,52E+00 0 0 0 0,00E+00 0,00E+00 0,00E+00 0,00E+00
PERT MJ 3,93E+01 5,43E-01 -6,52E+00 0 0 0 2,90E-02 3,08E-06 9,14E-09 -1,90E+01
PENRE MJ 2,42E+02 5,23E+01 9,30E-02 0 0 0 2,02E+00 5,53E-05 1,31E-07 -1,39E+02
PENRM MJ 4,69E+00 0,00E+00 0,00E+00 0 0 0 0,00E+00 -4,69E+00 0,00E+00 -4,34E+00
PENRT MJ 2,47E+02 5,23E+01 9,30E-02 0 0 0 2,02E+00 -4,68E+00 1,31E-07 -1,44E+02
SM kg 3,52E-01 0,00E+00 0,00E+00 0 0 0 0,00E+00 0,00E+00 0,00E+00 -7,41E-03
RSF MJ 7,84E-02 1,70E-02 5,08E-05 0 0 0 1,04E-03 6,61E-08 2,26E-10 7,94E-02
NRSF MJ 5,54E+00 1,07E-01 2,09E-04 0 0 0 3,70E-03 0,00E+00 2,14E-08 2,81E+00
FW m3 2,34E-01 4,16E-03 4,39E-05 0 0 0 2,16E-04 4,68E-07 1,21E-10 -1,32E-01
PERE = Use of renewable primary energy excluding renewable primary energy resources used as raw materials; PERM = Use of renewable primary energy resources used
as raw materials; PERT = Total use of renewable primary energy resources; PENRE = Use of non renewable primary energy excluding non-renewable primary energy
resources used as raw materials; PENRM = Use of non renewable primary energy resources used as raw materials; PENRT = Total use of non renewable primary energy
resources; SM = Use of secondary materials; RSF = Use of renewable secondary fuels; NRSF = Use of non-renewable secondary fuels; FW = Net use of fresh water
"Reading example: 9,0 E-03 = 9,0*10-3 = 0,009"
*INA Indicator Not Assessed
9 / 12
End of life - Waste
Indicator Unit A1-A3 A4 A5 B2 B6 C1 C2 C3 C4 D
HWD kg 5,50E-01 2,55E-03 0,00E+00 0 0 0 1,04E-04 0,00E+00 1,58E-07 -4,01E-01
NHWD kg 1,49E+01 1,34E+00 4,11E-01 0 0 0 9,84E-02 0,00E+00 1,51E-07 -1,17E+01
RWD kg 1,03E+01 3,59E-04 0,00E+00 0 0 0 1,38E-05 0,00E+00 1,00E-12 -1,03E+01
HWD = Hazardous waste disposed; NHWD = Non-hazardous waste disposed; RWD = Radioactive waste disposed
"Reading example: 9,0 E-03 = 9,0*10-3 = 0,009"
*INA Indicator Not Assessed
End of life - Output flow
Indicator Unit A1-A3 A4 A5 B2 B6 C1 C2 C3 C4 D
CRU kg 0,00E+00 0,00E+00 0,00E+00 0 0 0 0,00E+00 0,00E+00 0,00E+00 0,00E+00
MFR kg 1,54E-02 0,00E+00 3,82E-01 0 0 0 0,00E+00 9,22E+00 0,00E+00 -9,97E-04
MER kg 2,78E-01 0,00E+00 7,70E-04 0 0 0 0,00E+00 1,70E-04 0,00E+00 -1,20E-04
EEE MJ 1,69E-01 0,00E+00 2,35E-02 0 0 0 0,00E+00 2,61E-04 0,00E+00 -7,57E-04
EET MJ 2,55E+00 0,00E+00 3,56E-01 0 0 0 0,00E+00 3,95E-03 0,00E+00 -1,15E-02
CRU = Components for re-use; MFR = Materials for recycling; MER = Materials for energy recovery; EEE = Exported energy electrical; EET = Exported energy thermal
"Reading example: 9,0 E-03 = 9,0*10-3 = 0,009"
*INA Indicator Not Assessed
Biogenic Carbon Content
Indicator Unit At the factory gate
Biogenic carbon content in product kg C 0,00E+00
Biogenic carbon content in accompanying packaging kg C 1,90E-01
Note: 1 kg biogenic carbon is equivalent to 44/12 kg CO2
10 / 12
Additional requirements
Greenhouse gas emissions from the use of electricity in the manufacturing phase
National production mix from import, low voltage (production of transmission lines, in addition to direct emissions and losses in grid) of applied
electricity for the manufacturing process (A3).
Electricity mix Source Amount Unit
Electricity, photovoltaic, single-Si panel - China (kWh) ecoinvent 3.6 93,97 g CO2-eq/kWh
Dangerous substances
The product contains dangerous substances, more than 0,1% by weight, given by the REACH Candidate List, see table:
Name CASNo Amount
ISO 14025:2010 Environmental labels and declarations - Type III environmental declarations -
Lead >0,1
Principles and procedures, ISO 14044:2006 Environmental m
Indoor environment
Not applicable.
Additional Environmental Information
Additional environmental impact indicators required in NPCR Part A for construction products
Indicator Unit A1-A3 A4 A5 B2 B6 C1 C2 C3 C4 D
GWPIOBC kg CO2 -eq 2,14E+01 3,76E+00 6,65E-03 0 0 0 1,34E-01 4,02E-04 5,04E-07 -1,33E+01
GWP-IOBC: Global warming potential calculated according to the principle of instantaneous oxidation. In order to increase the transparency of biogenic carbon​
contribution to climate impact, the indicator GWP-IOBC is required as it declares climate impacts calculated according to the principle of instantaneous oxidation.​
GWP-IOBC is also referred to as GWP-GHG in context to Swedish public procurement legislation.
11 / 12
Bibliography
ISO 14025:2010 Environmental labels and declarations - Type III environmental declarations - Principles and procedures.
ISO 14044:2006 Environmental management - Life cycle assessment - Requirements and guidelines.
EN 15804:2012+A2:2019 Environmental product declaration - Core rules for the product category of construction products.
ecoinvent v3, Allocation, cut-off by classification, Swiss Centre of Life Cycle Inventories.
Iversen et al., (2021) eEPD v2021.09 Background information for EPD generator tool system verification, LCA.no Report number: 07.21
Ferreira, P. and Ruud, C.E., (2024) EPD generator for PCR 2010:08 Other Special- And General-Purpose Machinery and Parts Thereof: Background
information for EPD generator application and LCA data, LCA.no report number: 15.24
NPCR Part A: Construction products and services. Ver. 2.0. April 2021, EPD-Norge.
PCR 2010:08 for other special- and general-purpose machinery and parts thereof., ver. 4.0, 04.04.2022. The International EPD® System.
EN 50693:2019 Product category rules for life cycle assessments of electronic and electrical products and systems
General Programme Instructions for The Norwegian EPD Foundation/EPD-Norge (www.epd-norge.no) version 3:2019 updated 25/05/23.
Program operator and publisher Phone: +47 977 22 020
The Norwegian EPD Foundation e-mail: post@epd-norge.no
Post Box 5250 Majorstuen, 0303 Oslo, Norway web: www.epd-norge.no
Owner of the declaration: Phone: +46(0)31-7991600
GPBM Nordic AB e-mail: info@gpbmnordic.se
Sörredsvägen 113, 41878 Göteborg, Sweden web: https://www.gpbmnordic.no/
Author of the Life Cycle Assessment Phone: +47 916 50 916
LCA.no AS e-mail: post@lca.no
Dokka 6A, 1671 Kråkerøy, Norway web: www.lca.no
Developer of EPD generator Phone: +47 916 50 916
LCA.no AS e-mail: post@lca.no
Dokka 6A, 1671 Kråkerøy, Norway web: www.lca.no
ECO Platform web: www.eco-platform.org
ECO Portal web: ECO Portal
12 / 12
