Environmental product declaration
In accordance with ISO 14025 and EN 15804 +A2
i10-1500 LED 16000 HF 840 MB
Owner of the declaration: Program operator:
Glamox AS The Norwegian EPD Foundation
Declared unit: Declaration number:
1 pcs i10-1500 LED 16000 HF 840 MB
NEPD-3958-2994-EN
This declaration is based on Product Category Rules:
CEN Standard EN 15804:2012+A2:2019 serves as core PCR Registration number:
IBU PCR - Part B for luminaires, lamps, and components for
luminaires NEPD-3958-2994-EN
Issue date: 29.11.2022
Valid to: 29.11.2027
The Norwegian EPD Foundation
EPD Software:
LCA.no EPD generator
System ID:
53832
1 / 14
General information
Product Owner of the declaration:
i10-1500 LED 16000 HF 840 MB Glamox AS
Contact person: Birger Holo
Phone: +47 97551574
e-mail: birger.holo@glamox.com
Program operator: Manufacturer:
Post Box 5250 Majorstuen, 0303 Oslo, Norway Glamox AS
The Norwegian EPD Foundation Birger Hatlebakks veg 15 , 6415 Molde
Phone: +47 23 08 80 00 Global
web: post@epd-norge.no
Declaration number: Place of production:
NEPD-3958-2994-EN ​
Birger Hatlebakks veg 15 , 6415 Molde
Norway
GMlaamnaogxe pmroednut cstyisotne msit:e Molde (Norway
This declaration is based on Product Category Rules: ISO 9001, ISO 14001
CEN Standard EN 15804:2012+A2:2019 serves as core PCR
IBU PCR - Part B for luminaires, lamps, and components for luminaires
Organisation no:
Statement of liability: 912007782
The owner of the declaration shall be liable for the underlying information and
evidence. EPD Norway shall not be liable with respect t​o manufacturer
information, life cycle assessment data and evidences.
Issue date: 29.11.2022
Declared unit:
1 pcs i10-1500 LED 16000 HF 840 MB
Valid to: 29.11.2027
Declared unit with option:
A1,A2,A3,A4,A5,B6,C1,C2,C3,C4,D
Year of study:
Functional unit: 2022
1 pc i10-1500 LED luminaire manufactured in Glamox Molde. Transport to
costumer, installed and used according to a specific lighting regime over 20-years
lifetime. Including waste treatment at end-of-life.
Comparability:
General information on verification of EPD from EPD tools: EPD of construction products may not be comparable if they not comply with
Independent verification of data, other environmental information and the EN 15804 and seen in a building context.
declaration according to ISO 14025:2010, § 8.1.3 and § 8.1.4. Individualthird party
verification of each EPD is not required when the EPD tool is i) integrated into the
company's environmental management system, ii) the procedures for use of the
EPD tool are approved by EPDNorway, and iii)the proccess is reviewed annualy.
See Appendix G of EPD-Norway's General Programme Instructions for further
information on EPD tools.
Development and verification of EPD:
Verification of EPD tool: The declaration is created using EPD tool lca.tools ver EPD2021.09, developed by
Independent third party verification of the EPD tool, background data and test- LCA.no. The EPD tool is integrated in the company's management system, and
EPD in accordance with EPDNorway's procedures and guidelines for verification has been approved by EPD Norway.
and approval of EPD tools. Approval number: NEPDT41.
Developer of EPD:
Third party verifier:
Marthe Øyen Gaasø
Reviewer of company-specific input data and EPD:​
Vito D’Incognito - Take Care International Jonny Strømme
(no signature required)
Approved:
2 / 14
Product
Product description:
i10 is a IP23 luminaire with different lumen packages and types of reflectors in silver coated aluminium giving high flexibility. The luminaire housing is manufactured in
unpainted aluzink coated steel.
Product specification
Optic Name: MB - Medium beam. Reflector Material: Silver-coated aluminium. Certification: ENEC
Length 1,559mm. Width 161mm. Height 136mm.
Materials kg %
Electronic - Cable and connector 0,04 1,27
Electronic - LED driver 0,28 9,52
Electronic - LED plate 0,09 2,88
Electronic - Light emitting diode 0,00 0,13
Electronic - Resistor 0,00 0,00
Metal - Aluminium 0,39 13,13
Metal - Stainless steel 0,02 0,67
Metal - Steel 1,68 56,26
Plastic - Acrylonitrile butadiene styrene (ABS) 0,07 2,41
Plastic - Plexiglass (PMMA) 0,40 13,47
Rubber, synthetic 0,01 0,20
Silicon products 0,00 0,04
Total 2,98
Packaging kg %
Packaging - Paper 0,28 65,74
Packaging - Plastic 0,08 18,75
Packaging - Polystyrene 0,07 15,51
Total incl. packaging 3,42
Technical data:
Electrical Data: 1 Fixed output (HF) LED Driver. 220-240V 50-60Hz.
Total Consumption: 113W. Lumen Out: 16031. lm Lumen Per Watt:151lm/W.
Lamp colour temp (K): 4000. Colour Rendering Index: 80. MacAdams Step: 3. Leakage Current (mA):0.30. Energy Class Light Source C. Certification: ENEC
Minimum TA -25ºC Maximum TA 35ºC.
Market:
Norway
Reference service life, product
20 years.
LED Lifetime L80B50 Ta25 (h): 100 000. LED Lifetime L70B50 Max Ta (h): 90 000.
Reference service life, building or construction works
60 years.
Standard service life for buildings according to PCR Part A of EPD Norway.
LCA: Calculation rules
Declared unit:
1 pcs i10-1500 LED 16000 HF 840 MB
Cut-off criteria:
All major raw materials and all the essential energy is included. The production processes for raw materials and energy flows with very small amounts (less than 1%) can
be excluded. These cut-off criteria do not apply for hazardous materials and substances.
Allocation:
The allocation is made in accordance with the provisions of EN 15804. Incoming energy and water and waste production in-house is allocated equally among all products
through mass allocation. Effects of primary production of recycled materials is allocated to the main product in which the material was used. The recycling process and
transportation of the material is allocated to this analysis.
Data quality:
Specific data for the product composition are provided by the manufacturer. The data represent the production of the declared product and were collected for EPD
development in the year of study. Background data is based on EPDs according to EN 15804 and different LCA databases. The data quality of the raw materials in A1 is
presented in the table below.
3 / 14
Materials Source Data quality Year
Electronic - Cable and connector ecoinvent 3.6 Database 2019
Electronic - LED plate ecoinvent 3.6 Database 2019
Electronic - Resistor ecoinvent 3.6 Database 2019
Metal - Aluminium ecoinvent 3.6 Database 2019
Metal - Stainless steel ecoinvent 3.6 Database 2019
Metal - Steel ecoinvent 3.6 Database 2019
Packaging - Paper ecoinvent 3.6 Database 2019
Packaging - Plastic ecoinvent 3.6 Database 2019
Packaging - Polystyrene ecoinvent 3.6 Database 2019
Plastic - Acrylonitrile butadiene styrene (ABS) ecoinvent 3.6 Database 2019
Plastic - Plexiglass (PMMA) ecoinvent 3.6 Database 2019
Rubber, synthetic ecoinvent 3.6 Database 2019
Silicon products ecoinvent 3.6 Database 2019
Database;
Electronic - Cable and connector ecoinvent 3.6; manufacturer 2019
technical sheet
LCA literature;
Electronic - Light emitting diode Scholand et al. (2012); Ecoinvent 3.6 2019
database
Supplier
Electronic - LED driver ecoinvent 3.6 2019
specific/database
Metal - Steel EPD S-P-01921; ecoinvent 3.6 EPD; database 2020
4 / 14
System boundaries (X=included, MND=module not declared, MNR=module not relevant)
Construction Beyond the
Product stage installation Use stage End of life stage system
stage boundaries
A1 A2 A3 A4 A5 B1 B2 B3 B4 B5 B6 B7 C1 C2 C3 C4 D
X X X X X MND MND MND MND MND X MND X X X X X
System boundary:
The analysis is a cradle-to-grave study of one luminaire manufactured and installed, used according to a specific lighting regime over a specific lifetime, including waste
treatment at end-of-life.
A1-A5 includes the extraction and production of raw materials, transportation to the production site, the production process itself, transport to the market and assembly.
B6 is the operational energy use stage of the luminaire based on a scenario.
C1-C4 includes de-installation of the luminaire, average transport between building site and waste treatment facility, waste processing and disposal. Waste treatment of
the product follows the default values provided in EN 50693.
D shows the recyclability of metals and plastics, and allows the producers a credit for the net scrap that is produced at the end of a product’s life. The benefits from
recycling of net scrap are described in formula from EN 15804:2012+A2:2019. Substitution of heat and electricity generated by the incineration with energy recovery of
plastic insulation and other parts is also calculated in module D.
The flowchart in the figure below illustrates the system boundaries for the analysis.
Additional technical information:
Please visit our website www.glamox.com for more technical information.
waR slairetam tropsnarT gnirutcafunaM tropsnarT ylbmessA e​sU ecnanetniaM riapeR tnemecalpeR tnemhsibrufeR lanoitarepO esu ygrene lanoitarepO esu retaw -eD noitcurtsnoc noitilomed tropsnarT etsaW gnissecorp lasopsiD -yrevoceR-esueR -gnilcyceR laitnetop
5 / 14
LCA: Scenarios and additional technical information
The following information describe the scenarios in the different modules of the EPD.
Module A4 = Transport from manufacturing location in Molde to warehouse in Oslo (495 km) + average distribution into the Norwegian market (300 km)
Module B6 = The operational energy use of the luminaire is calculated based on the methodology provided in IBU PCR Part B for luminaires, lamps, and components for
luminaires. The energy consumption model for luminaire used in the PCR follows the application scenarios developed in EN 15193:2007. To calculate the electricity use of
the luminaire, the following scenario parameters have been applied:
- Active power of the luminaire (Pa) = 113 watt
- Passive power of the luminaire (Pp) = 0 watt
- Daylight time usage (tD) = 2500 hours
- Non-daylight time usage (tN) = 1500 hours
- Standard year time (ty) = 8760 hours
- The occupancy depency factor (FO) = 1 (factor, no unit)
- The daylight dependency factor (FD) = 1 (factor, no unit)
- The product specific constant illuminance factor (FCP) = 1 (factor, no unit)
- The non-daylight dimming factor (FN) = 1 (factor, no unit)
- The application specific empiric lifetime of the luminaire in years (a) = 20 years (corresponding to the reference service life of the product).
Module C2 = Average transport to Norwegian waste treatment facilities.
Modules C3 and C4 = Waste treatment of the product follows the default values provided in EN 50693, Product Category Rules for life cycle assessments of electronic and
electrical products and systems, table G.4. This table specified how different types of raw materials used in A1 will likely be treated during the end-of-life of the product.
Waste treatments in C3 include material recycling and incineration with and without energy recovery and fly ash extraction. Disposal in C4 consist of landfilling of
different waste fractions and of ashes.
Module D = The recyclability of metals, plastics, and electronic components allows the producers a credit for the net scrap that is produced at the end of a product’s life.
The benefits from recycling of net scrap are described in formula from EN 15804:2012+A2:2019. Substitution of heat and electricity generated by the incineration with
energy recovery of plastic insulation and other parts is also calculated in module D.
Capacity utilisation Value
Transport from production place to user (A4) Distance (km) Fuel/Energy Consumption Unit
(incl. return) % (Liter/tonne)
Truck, 16-32 tonnes, EURO 5 (km) 36,7 % 795 0,044 l/tkm 34,98
Assembly (A5) Unit Value
Waste, cardboard and paper, to average treatment
kg 0,28
- A5 including transport (kg)
Waste, plastic, mixture, to average treatment - A5
kg 0,15
including transport (kg)
Operational energy (B6) Unit Value
Electricity, Norway (kWh) kWh/DU 9040,00
Capacity utilisation Value
Transport to waste processing (C2) Distance (km) Fuel/Energy Consumption Unit
(incl. return) % (Liter/tonne)
Truck, over 32 tonnes, EURO 5 (km) 53,3 % 300 0,023 l/tkm 6,90
Waste processing (C3) Unit Value
Acrylonitrile butadiene styrene (ABS) to recycling kg 0,01
Aluminium to recycling (kg) kg 0,27
Copper to recycling (kg) kg 0,01
Steel to recycling (kg) kg 1,41
Waste treatment of non-hazardous waste,
incineration with energy recovery and fly ash kg 0,00
extraction (kg)
Waste treatment of plastic mixture, incineration
kg 0,28
with energy recovery and fly ash extraction (kg)
Waste treatment per kg electronics scrap from
PWB, with components, recycling of metals, lead- kg 0,08
free - C3 (kg)
Waste treatment per kg electronics scrap from
PWB, without components, recycling of copper - kg 0,04
C3 (kg)
Waste treatment per kg used electronic cable,
kg 0,02
manual seperation (kg)
Waste treatment per kg used electronic LED driver,
kg 0,28
manual seperation (kg)
Waste treatment per kg used electronic plug
kg 0,01
connector, manual seperation (kg)
Waste treatment per kg used PWB, shredding and
kg 0,25
separation - C3 (kg)
6 / 14
Disposal (C4) Unit Value
Landfilling of aluminium (kg) kg 0,12
Landfilling of ashes from incineration of Non-
hazardous waste, process per kg ashes and kg 0,00
residues (kg)
Landfilling of ashes from incineration of Plastic
kg 0,01
mixture, process per kg ashes and residues (kg)
Landfilling of copper (kg) kg 0,01
Landfilling of hazardous waste (kg) kg 0,13
Landfilling of non-hazardous waste (kg) kg 0,00
Landfilling of plastic mixture (kg) kg 0,28
Landfilling of steel (kg) kg 0,35
Benefits and loads beyond the system
Unit Value
boundaries (D)
Substitution of primary copper with net scrap
g 29,23
from printed wiring board (g)
Substitution of primary gold with net scrap from
g 0,01
printed wiring board (g)
Substitution of primary nickel with net scrap from
g 2,66
printed wiring board (g)
Substitution of primary palladium with net scrap
g 0,02
from printed wiring board (g)
Substitution of primary silver with net scrap from
g 0,45
printed wiring board (g)
Substitution of acrylonitrile butadiene styrene,
kg 0,01
ABS, granulate (kg)
Substitution of primary aluminium with net scrap
kg -0,04
(kg)
Substitution of primary copper with net scrap (kg) kg 0,01
Substitution of primary steel with net scrap (kg) kg 0,21
Substitution of electricity, in Norway (MJ) MJ 0,43
Substitution of thermal energy, district heating, in
MJ 6,49
Norway (MJ)
7 / 14
LCA: Results
The LCA results are presented below for the declared unit defined on page 2 of the EPD document.
Environmental impact
Parameter Unit A1 A2 A3 A4 A5
GWP-total kg CO2 -eq 4,25E+01 4,44E-01 4,13E-01 4,54E-01 5,12E-01
GWP-fossil kg CO2 -eq 4,26E+01 4,44E-01 3,89E-01 4,53E-01 1,63E-02
GWP-biogenic kg CO2 -eq -2,27E-01 1,75E-04 2,25E-02 1,85E-04 4,95E-01
GWP-luluc kg CO2 -eq 6,77E-02 1,65E-04 1,13E-03 1,58E-04 2,42E-06
ODP kg CFC11 -eq 2,84E-06 1,00E-07 2,69E-08 1,03E-07 1,67E-09
AP mol H+ -eq 3,40E-01 2,87E-03 4,02E-03 1,85E-03 3,62E-05
EP-FreshWater kg P -eq 5,04E-03 3,34E-06 2,04E-05 3,56E-06 6,18E-08
EP-Marine kg N -eq 4,76E-02 7,95E-04 1,18E-03 5,49E-04 2,04E-05
EP-Terrestial mol N eq 7,03E-01 8,81E-03 1,31E-02 6,08E-03 1,30E-04
POCP kg NMVOC -eq 1,75E-01 2,54E-03 3,54E-03 1,86E-03 3,94E-05
ADP-minerals&metals1 Kg Sb-eq 1,40E-02 1,13E-05 2,10E-05 1,23E-05 1,74E-07
ADP-fossil1 MJ 5,51E+02 6,61E+00 4,49E+00 6,83E+00 1,13E-01
WDP1 m3 1,93E+03 5,94E+00 6,37E+02 6,52E+00 2,52E-01
Parameter Unit B6 C1 C2 C3 C4 D
GWP-total kg CO2 -eq 2,20E+02 0,00E+00 9,33E-02 7,53E-01 6,64E-02 -1,35E+00
GWP-fossil kg CO2 -eq 2,13E+02 0,00E+00 9,32E-02 7,51E-01 6,56E-02 -1,35E+00
GWP-biogenic kg CO2 -eq 5,89E+00 0,00E+00 3,83E-05 1,21E-03 5,19E-04 -2,82E-03
GWP-luluc kg CO2 -eq 8,79E-01 0,00E+00 2,72E-05 2,24E-04 2,42E-04 3,46E-03
ODP kg CFC11 -eq 1,46E-05 0,00E+00 2,15E-08 7,03E-09 4,14E-09 -2,74E-03
AP mol H+ -eq 1,67E+00 0,00E+00 3,92E-04 4,97E-04 2,01E-04 -9,08E-02
EP-FreshWater kg P -eq 1,53E-02 0,00E+00 7,11E-07 2,91E-06 1,36E-06 -5,23E-04
EP-Marine kg N -eq 1,83E-01 0,00E+00 1,18E-04 1,33E-04 8,61E-05 -4,66E-03
EP-Terrestial mol N eq 2,38E+00 0,00E+00 1,30E-03 1,43E-03 5,72E-04 -6,43E-02
POCP kg NMVOC -eq 6,41E-01 0,00E+00 4,19E-04 3,76E-04 2,26E-04 -1,86E-02
ADP-minerals&metals1 Kg Sb-eq 1,59E-02 0,00E+00 1,59E-06 7,42E-07 2,29E-07 -2,00E-03
ADP-fossil1 MJ 2,91E+03 0,00E+00 1,45E+00 9,71E-01 5,18E-01 -1,71E+01
WDP1 m3 5,07E+05 0,00E+00 1,11E+00 9,54E+00 4,83E+00 1,72E+02
GWP total Global Warming Potential total; GWP fossil Global Warming Potential fossil fuels ; GWP biogenic Global Warming Potential biogenic; GWP luluc Global W
Potential land use change; ODP Ozone Depletion; AP Acidification; EP freshwater Eutrophication aquatic freshwater; EP marine Eutrophication aquatic marine; EP
terrestrial Eutrophication terrestrial ;POCP Photochemical zone formation; ADPE Abiotic Depletion Potential minerals and metals; ADPf Abiotic Depletion Potential fossil
fuels;
"Reading example: 9,0 E-03 = 9,0*10-3 = 0,009"
*INA Indicator Not Assessed
1. The results of this environmental impact indicator shall be used with care as the uncertainties on these results are high or as there is limited experienced with the
indicator
Remarks to environmental impacts
A luminaire is a product that consumes energy during the use phase. Combined with a relatively long expected lifetime and the environmental impact of generating
electricity, the use phase (B6) will normally be the most contributing stage to the overall environmental impact of the declared unit. It is important to be aware that the
actual calculations of the effect of B6 is particularly sensitive to which use scenario that is chosen and which energy grid mix that is used.
8 / 14
Additional environmental impact indicators
Parameter Unit A1 A2 A3 A4 A5
PM Disease incidence 2,88E-06 3,03E-08 6,99E-08 3,26E-08 5,81E-10
IRP2 kgBq U235 eq. 1,86E+00 2,88E-02 6,85E-02 2,99E-02 4,93E-04
ETP-fw1 CTUe 2,34E+03 4,79E+00 1,78E+01 5,03E+00 1,32E-01
HTP-c1 CTUh 8,07E-08 0,00E+00 8,71E-10 0,00E+00 4,00E-12
HTP-nc1 CTUh 1,96E-06 5,22E-09 2,08E-08 5,44E-09 1,52E-10
SQP1 Pt 2,06E+02 4,29E+00 2,18E+00 4,71E+00 1,27E-01
Parameter Unit B6 C1 C2 C3 C4 D
PM Disease incidence 1,19E-05 0,00E+00 8,21E-09 3,06E-09 3,65E-09 -1,97E-07
IRP2 kgBq U235 eq. 5,28E+01 0,00E+00 6,34E-03 4,82E-03 1,80E-03 -4,84E-02
ETP-fw1 CTUe 1,33E+04 0,00E+00 1,06E+00 2,98E+00 2,94E+02 -6,79E+02
HTP-c1 CTUh 6,33E-07 0,00E+00 0,00E+00 1,51E-09 1,34E-10 -3,99E-09
HTP-nc1 CTUh 1,49E-05 0,00E+00 1,03E-09 8,87E-08 1,13E-09 -2,46E-07
SQP1 Pt 1,47E+03 0,00E+00 1,66E+00 2,31E-01 1,27E+00 -1,74E+01
PM Particulate Matter emissions; IRP Ionizing radiation – human health; ETP-fw Eco toxicity – freshwater; HTP-c Human toxicity – cancer effects; HTP-nc Human
toxicity – non cancer effects; SQP Soil Quality (dimensionless)
"Reading example: 9,0 E-03 = 9,0*10-3 = 0,009"
*INA Indicator Not Assessed
1. The results of this environmental impact indicator shall be used with care as the uncertainties on these results are high or as there is limited experienced with the
indicator
2. This impact category deals mainly with the eventual impact of low dose ionizing radiation on human health of the nuclear fuel cycle. It does not consider effects due
to possible nuclear accidents, occupational exposure nor due to radioactive waste disposal in underground facilities. Potential ionizing radiation from the soil, from
radon and from some construction materials is also not measured by this indicator.
9 / 14
Resource use
Parameter Unit A1 A2 A3 A4 A5
PERE MJ 5,19E+01 8,95E-02 4,72E+01 9,64E-02 2,28E-03
PERM MJ 1,13E+01 0,00E+00 0,00E+00 0,00E+00 -1,13E+01
PERT MJ 6,32E+01 8,95E-02 4,72E+01 9,64E-02 -1,13E+01
PENRE MJ 5,25E+02 6,61E+00 4,50E+00 6,83E+00 1,13E-01
PENRM MJ 2,57E+01 0,00E+00 0,00E+00 0,00E+00 -6,03E+00
PENRT MJ 5,51E+02 6,61E+00 4,50E+00 6,83E+00 -5,92E+00
SM kg 1,97E+00 0,00E+00 5,45E-02 0,00E+00 8,82E-05
RSF MJ 9,82E-01 3,17E-03 3,77E-02 3,45E-03 6,71E-05
NRSF MJ 3,65E+00 1,01E-02 9,80E-02 1,23E-02 2,28E-04
FW m3 4,28E-01 6,69E-04 3,53E-01 7,20E-04 5,59E-05
Parameter Unit B6 C1 C2 C3 C4 D
PERE MJ 3,77E+04 0,00E+00 1,83E-02 1,37E-01 1,29E-01 -3,62E+00
PERM MJ 0,00E+00 0,00E+00 0,00E+00 0,00E+00 0,00E+00 0,00E+00
PERT MJ 3,77E+04 0,00E+00 1,83E-02 1,37E-01 1,29E-01 -3,62E+00
PENRE MJ 2,91E+03 0,00E+00 1,45E+00 9,71E-01 5,18E-01 -1,71E+01
PENRM MJ 0,00E+00 0,00E+00 0,00E+00 -2,16E+01 0,00E+00 0,00E+00
PENRT MJ 2,91E+03 0,00E+00 1,45E+00 -2,06E+01 5,18E-01 -1,94E+01
SM kg 0,00E+00 0,00E+00 0,00E+00 1,32E-04 5,21E-03 6,45E-02
RSF MJ 2,96E+01 0,00E+00 6,39E-04 2,12E-03 7,38E-04 -2,00E-02
NRSF MJ 7,37E+01 0,00E+00 2,14E-03 -1,16E-03 2,36E-02 3,97E-02
FW m3 2,82E+02 0,00E+00 1,65E-04 1,42E-03 4,45E-04 -9,92E-03
PERE Use of renewable primary energy excluding renewable primary energy resources used as raw materials; PERM Use of renewable primary energy resources used as
raw materials; PERT Total use of renewable primary energy resources; PENRE Use of non renewable primary energy excluding non-renewable primary energy resources
used as raw materials; PENRM Use of non renewable primary energy resources used as raw materials; PENRT Total use of non renewable primary energy resources; SM
Use of secondary materials; RSF Use of renewable secondary fuels; NRSF Use of non renewable secondary fuels; FW Use of net fresh water
"Reading example: 9,0 E-03 = 9,0*10-3 = 0,009"
*INA Indicator Not Assessed
10 / 14
End of life - Waste
Parameter Unit A1 A2 A3 A4 A5
HWD kg 2,38E-01 3,32E-04 2,98E-02 3,49E-04 3,03E-04
NHWD kg 6,55E+00 2,94E-01 3,25E-01 3,27E-01 7,67E-02
RWD kg 1,50E-03 4,51E-05 3,58E-05 4,66E-05 7,50E-07
Parameter Unit B6 C1 C2 C3 C4 D
HWD kg 1,87E+00 0,00E+00 7,94E-05 2,60E-04 1,45E-01 -8,05E-03
NHWD kg 2,24E+02 0,00E+00 1,26E-01 6,35E-02 7,66E-01 -2,47E-01
RWD kg 2,61E-02 0,00E+00 9,90E-06 4,17E-06 2,02E-06 -4,02E-05
HWD Hazardous waste disposed; NHWD Non-hazardous waste disposed; RWD Radioactive waste disposed;
"Reading example: 9,0 E-03 = 9,0*10-3 = 0,009"
*INA Indicator Not Assessed
End of life - Output flow
Parameter Unit A1 A2 A3 A4 A5
CRU kg 0,00E+00 0,00E+00 0,00E+00 0,00E+00 0,00E+00
MFR kg 4,89E-03 0,00E+00 1,02E+00 0,00E+00 3,40E-01
MER kg 3,94E-04 0,00E+00 6,35E-06 0,00E+00 7,24E-07
EEE MJ 4,10E-03 0,00E+00 1,22E-01 0,00E+00 1,72E-02
EET MJ 6,21E-02 0,00E+00 1,85E+00 0,00E+00 2,60E-01
Parameter Unit B6 C1 C2 C3 C4 D
CRU kg 0,00E+00 0,00E+00 0,00E+00 0,00E+00 0,00E+00 0,00E+00
MFR kg 0,00E+00 0,00E+00 0,00E+00 1,70E+00 2,73E-03 6,51E-02
MER kg 0,00E+00 0,00E+00 0,00E+00 2,19E-05 6,36E-05 5,78E-05
EEE MJ 0,00E+00 0,00E+00 0,00E+00 4,29E-01 5,89E-04 -2,74E-03
EET MJ 0,00E+00 0,00E+00 0,00E+00 6,49E+00 8,91E-03 -4,15E-02
CRU Components for re-use; MFR Materials for recycling; MER Materials for energy recovery; EEE Exported electrical energy; EET Exported Energy Thermal
"Reading example: 9,0 E-03 = 9,0*10-3 = 0,009"
*INA Indicator Not Assessed
Biogenic Carbon Content
Parameter Unit At the factory gate
Biogenic carbon content in product kg C 0,00E+00
Biogenic carbon content in accompanying packaging kg C 1,35E-01
Note: 1 kg biogenic carbon is equivalent to 44/12 kg CO2
11 / 14
Additional Norwegian requirements
Greenhouse gas emissions from the use of electricity in the manufacturing phase
National production mix from import, low voltage (production of transmission lines, in addition to direct emissions and losses in grid) of applied electricity for the
manufacturing process (A3).
Electricity mix Data source Amount Unit
Electricity, Norway (kWh) ecoinvent 3.6 24,33 g CO2-eq/kWh
Dangerous substances
The product contains no substances given by the REACH Candidate list or the Norwegian priority list.
Indoor environment
Not relevant.
Additional Environmental Information
Environmental impact indicators EN 15804+A1 and NPCR Part A v2.0
Parameter Unit A1 A2 A3 A4 A5
GWP kg CO2 -eq 4,11E+01 4,39E-01 3,94E-01 4,49E-01 5,09E-01
ODP kg CFC11 -eq 2,95E-06 7,93E-08 3,06E-08 8,16E-08 1,35E-09
POCP kg C2H4-eq 2,03E-02 7,86E-05 1,07E-04 5,99E-05 2,13E-06
AP kg SO2 -eq 2,35E-01 1,76E-03 1,80E-03 8,90E-04 1,79E-05
EP kg PO43- -eq 3,17E-02 1,91E-04 1,96E-04 9,50E-05 6,68E-06
ADPM kg Sb -eq 1,40E-02 1,13E-05 2,10E-05 1,23E-05 1,74E-07
ADPE MJ 4,75E+02 6,48E+00 2,60E+00 6,69E+00 1,10E-01
GWPIOBC kg CO2 -eq 4,30E+01 4,44E-01 3,02E-01 4,54E-01 0,00E+00
Parameter Unit B6 C1 C2 C3 C4 D
GWP kg CO2 -eq 2,10E+02 0,00E+00 9,23E-02 7,51E-01 5,87E-02 -1,30E+00
ODP kg CFC11 -eq 1,86E-05 0,00E+00 1,74E-08 6,38E-09 3,79E-09 -6,92E-08
POCP kg C2H4-eq 6,26E-02 0,00E+00 1,20E-05 1,76E-05 2,39E-05 -3,03E-03
AP kg SO2 -eq 1,32E+00 0,00E+00 1,86E-04 3,80E-04 1,26E-04 -7,69E-02
EP kg PO43- -eq 1,23E-01 0,00E+00 2,03E-05 6,42E-05 3,23E-05 -3,16E-03
ADPM kg Sb -eq 1,59E-02 0,00E+00 1,59E-06 7,42E-07 2,32E-07 -2,00E-03
ADPE MJ 1,43E+03 0,00E+00 1,42E+00 8,35E-01 4,86E-01 -1,58E+01
GWPIOBC kg CO2 -eq 2,20E+02 0,00E+00 9,33E-02 7,53E-01 9,01E-03 -1,47E+00
GWP Global warming potential; ODP Depletion potential of the stratospheric ozone layer; POCP Formation potential of tropospheric photochemical oxidants; AP
Acidification potential of land and water; EP Eutrophication potential; ADPM Abiotic depletion potential for non fossil resources; ADPE Abiotic depletion​ potential for
fossil resources; GWP-IOBC/GHG Global warming potential calculated according to the principle of instantanious oxidation (except emissions and uptake of biogenic
carbon)
12 / 14
Bibliography
ISO 14025:2010. Environmental labels and declarations - Type III environmental declarations - Principles and procedures. International Organization for Standardization.
ISO 14044:2006. Environmental management - Life cycle assessment - Requirements and guidelines. International Organization for Standardization.
EN 15804:2012+A2:2019. Environmental product declaration - Core rules for the product category of construction products. European Committee for Standardization.
ISO 21930:2017. Sustainability in buildings and civil engineering works - Core rules for environmental product declarations of construction products. International
Organization for Standardization.
EN 50693:2019. Product category rules for life cycle assessments of electronic and electrical products and systems. European Committee for Standardization.
Ecoinvent v3, 2019. Allocation, cut-off by classification. Swiss Centre of Life Cycle Inventories.
Iversen et al., (2021). eEPD v2021.09, background information for EPD generator tool system verification, LCA.no. Report number: 07.21. System verification report.
Philis et al., (2022). EPD generator for IBU PCR part B for luminaires, lamps, and components for luminaires, background information for EPD generator application and
LCA data, LCA.no. Report number: 04.22. PCR verification report.
EPD Norway (2022). NPCR Part A: Construction products and services. The Norwegian EPD foundation. Version 2.0 published 24.03.2021.
IBU (2017). PCR part B for luminaires, lampes and components for luminaires. Institut Bauen und Umwelt e.V. Version 1.7, published 30.11.2017.
Life cycle inventory (LCI) report for i10-1500 LED 16000 HF 840 MB, Glamox, November 2022.
Program operator and publisher Phone: +47 23 08 80 00
The Norwegian EPD Foundation e-mail: post@epd-norge.no
Post Box 5250 Majorstuen, 0303 Oslo, Norway web: www.epd-norge.no
Owner of the declaration: Phone: +47 97551574
Glamox AS e-mail: birger.holo@glamox.com
Birger Hatlebakks veg 15, 6415 Molde web: https://www.glamox.com/no/pbs/
Author of the Life Cycle Assessment Phone: +47 916 50 916
LCA.no AS e-mail: post@lca.no
Dokka 6B, 1671 web: www.lca.no
Developer of EPD generator Phone: +47 916 50 916
LCA.no AS e-mail: post@lca.no
Dokka 6B,1671 Kråkerøy web: www.lca.no
ECO Platform Web: www.eco-platform.org
ECO Portal Web: ECO Portal
13 / 14
EPD for the best
environmental
decision
The Norwegian EPD Foundation
www.epd-norge.no
14 / 14
