ver1 2015
ENVIRONMENTAL PRODUCT DECLARATION
in accordance with ISO 14025, ISO 21930 and EN 15804
Saint-Gobain Sweden AB, ISOVER
Owner of the declaration:
Program operator: The Norwegian EPD Foundation
The Norwegian EPD Foundation
Publisher:
Declaration number: NEPD-2502-1244-EN
NEPD-2502-1244-EN
Registration number:
ECO Platform reference number: -
Issue date: 03.11.2020
Valid to: 03.11.2025
ISOVER Fasadskiva 30 Alu
Saint-Gobain Sweden AB
www.epd-norge.no
NEPD-2502-1244-EN ISOVER Fasadskiva 30 Alu
General information
Product Owner of the declaration
ISOVER Fasadskiva 30 Alu Saint-Gobain Sweden AB, ISOVER
Program operator Contact person: Daniel Odby
The Norwegian EPD Foundation Phone: +46 (0)42-842 52
Post Box 5250 Majorstuen, 0303 Oslo E-mail: daniel.odby@saint-gobain.com
Phone: +47 23 08 82 92
E-mail: post@epd-norge.no Manufacture
Web: www.epd-norge.no Saint-Gobain Sweden AB, ISOVER
Declaration number Place of production
Billesholm, Sweden
NEPD-2502-1244-EN
Management system
ECO Platform reference number SS-EN ISO 9001:2008
SS-EN ISO 14001:2004
This declaration is based on Product Category
Rules Org. No.
CEN Standard EN 15804 serve as core PCR. 556241-2592
The Product Category Rules, NPCR 012:2018 Part B
for Thermal insulation products is used in addition to Issue date 03.11.2020
the core PCR.
Statement of liability Valid to 03.11.2025
The owner of the declaration shall be liable for the
underlying information and evidence. EPD Norway shall
not be liable with respect to manufacturer information, Year of study
life cycle assessment data and evidences. 2018
Declared unit Comparability
1m² with a thermal resistance of 1,0 K.m²/W a thickness EPD of construction products may not be
of 30 mm. comparable if they do not comply with EN15804 and
seen in a building context.
Functional unit
1m² with a thermal resistance of 1,0 K.m²/W with a The EPD has been worked out by
reference service life of 60 years The EPD has been worked by the use of EPD tool,
GaBi, version 8.7 by Saint-Gobain LCA central
Verification team and by Malin Dalborg.
Independent verification of calculation data and other
environmental information and test of the computer Company specific LCA data has been worked out
program was carried out by Martin Erlandsson in by Patricia Jimenez Diaz, Saint-Gobain central
accordance with ISO14025, 8.1.3 and 8.1.4 + EN 15804 LCA team.
Approved
Externally
_________________________________________
IVL Swedish Environmental Research Institute
(Independent verifier approved by EPD Norway)
NEPD-2502-1244-EN ISOVER Fasadskiva 30 Alu
Product description
Product description and description of use:
This EPD describes the potential environmental impacts of 1 m² of glass wool insulation, ISOVER
Fasadskiva 30 Alu with a thermal resistance equal to 1 K.m².W-1. The intended use of this EPD is to
communicate scientifically based environmental information for construction products, for the purpose of
assessing the environmental performance of buildings.
ISOVER glass wool products are CE-marked according to the EN 13172 (2011) “Thermal Insulation Products
– Evaluation of Conformity”, EN 13162 (2012) “Thermal insulation Products for Buildings. Factory made
mineral wool (MW) Products. Specification” and EN 14303 “Thermal insulation products for building equipment
and industrial installations. Factory made mineral wool (MW) products. Specification”.
The production site of Saint-Gobain Sweden AB, ISOVER in Billesholm, uses a small amount of natural and
abundant raw materials (sand, soda, limestone, feldspar) and high share of recycled glass cullets (more than
50% post-consumer recycled content of the glass). This material is converted by using fusion and fiberizing
techniques to produce glass wool. The products obtained come in the form of a glass wool pipe section.
On Earth, naturally, the best insulator is dry immobile air at 10°C: its thermal conductivity factor,
expressed in λ, is 0.025 W/(m.K) (watts per meter Kelvin degree). The thermal conductivity of mineral wool at
10°C is close to immobile air as its lambda varies from 0.030 W/(m.K) for the most efficient to 0.040 W/(m.K). For
technical insulation the thermal conductivity is declared for different temperatures.
With its entangled structure, glass wool is a porous material that traps the air, making it one of the best
insulating materials. The porous and elastic structure of the wool also absorbs noise in the air and offers
acoustic correction inside premises. Glass wool mainly containing incombustible materials and does not
react to fire.
Glass wool insulation is used in buildings as well as industrial facilities. It ensures a high level of
comfort, minimizes carbon dioxide (CO ) emissions by preventing heat losses through roofs, walls,
2
floors, pipes and boilers. It reduces noise and protects homes and industrial facilities against fire.
Correctly installed glass wool products and solutions do not require maintenance and last throughout the
lifetime of the building (which is set at 60 years as a default value in the model), or as long as the insulated
building component is a part of the building.
2
NEPD-2502-1244-EN ISOVER Fasadskiva 30 Alu
Technical data/physical characteristics (for a thickness of 30 mm):
Thermal resistance of the Product: 1 K.m²/W (UNE EN 12667)
The thermal conductivity of the Glass wool is: 0.030 W/(m·K) at 10° (EN 14303)
Reaction to fire: A2-s1;d0
Description of the main product components and or materials:
Main components
Glass wool 90-95% (REACH registration number 01-2119472313-44-0041)
Binder 0-10%
Description of the main components and/or materials for 1 m² of product with a thermal resistance of 1
K.m2.W-1 a thickness of 30 mm for the calculation of the EPD®:
PARAMETER VALUE (per functional unit)
Quantity of wool for 1 m² of product 1.65 kg
Thickness of wool 30 mm
Surfacing Aluminum foil 85.0 g/m²
Polyethylene: 29.7 g/m²
Packaging for the transportation and distribution Wood pallet: 239.2 g/m²
Label: 0.120 g/m²
Product used for the Installation None
LCA calculation information
Providing a thermal insulation on 1 m² with a thermal
FUNCTIONALUNIT resistance of equals 1 K.m2.W-1
Cradle to Grave. Mandatory stages: A1-3, A4-5, B1- 7,
SYSTEM BOUNDARIES C1-4
REFERENCE SERVICELIFE(RSL) 60 years
CUT-OFFRULES See detailed explanation page 4
ALLOCATIONS See detailed explanation page 4
Renewable electricity mix (reference year 2018). This
100% renewable electricity bought is evidenced by
ELECTRICITY USED FOR THE
Guarantee of Origin certificates, GO’s, from LOS,
MANUFACTORING PROCESS
contracted 2018- 2020, to be prolonged to be valid at
least equal to the validity of this EPD.
GEOGRAPHICAL COVERAGE AND
Sweden 2018
TIME PERIOD
3
NEPD-2502-1244-EN ISOVER Fasadskiva 30 Alu
Cut-off criteria
The cut-off criterion used in Saint-Gobain EPD will be the mass criterion with the following details:
- Taking into account all input and output flows in a unit process i.e. taking into account the value of all
flows in the unit process and the corresponding LCI whenever available
- No simplification of the LCI by additional exclusions of material flows
Data collected at the manufacturing site was used. The inventory process in this LCA includes all data related
to raw material, packaging material and consumable items, and the associated transport to the manufacturing
site. Process energy and water use, direct production waste and emissions to air and water are included.
Scenarios have been developed to account for downstream processes such as demolition and waste treatment
in accordance with the requirements of EN 15804:2012+A1:2013
All inputs and outputs to the manufacturing plants have been included and made transparent. All assumptions
regarding the materials and water balances have also been included.
All hazardous and toxic materials and substances are considered in the inventory even though they are below
the cut off criteria
There are excluded processes in the inventory:
- Flows related to human activities such as employee transport and administration activity.
Allocation
Allocation criteria are based on mass.
The allocation of all the air emissions, wastes and energy usage are based on mass (kg). The reason we can
use a mass basis is because we use the exact same manufacturing process shown for every product. We only
produce glass mineral wool in the Billesholm site using the same process and therefore all the factors can be
allocated by a mass basis. The amount of binder varies for different products and is accounted for as well as if
different surface layers are used.
A mass balance was conducted for the 2018 production year to ensure that we have not excluded any materials,
emissions and hence potential environmental impacts. Regarding the mass balance, all the raw materials and
corresponding production goods and wastes generated were taken into account.
4
NEPD-2502-1244-EN ISOVER Fasadskiva 30 Alu
Flow diagram of the Life Cycle
5
NEPD-2502-1244-EN ISOVER Fasadskiva 30 Alu
System boundaries (X=included, MND=module not declared)
Beyond the
Construction
Product stage Use stage End of life stage system
installation stage
boundaries
6
slairetam
waR
tropsnarT
gnirutcafunaM
tropsnarT
noitallatsni
noitcurtsnoC
egats esU
ecnanetniaM
riapeR
tnemecalpeR tnemhsibrufeR
esu
ygrene
lanoitarepO
esu
retaw
lanoitarepO
noitcurtsnoc-eD
noitilomed tropsnarT
gnissecorp
etsaW
lasopsiD
-yrevoceR-esueR laitnetop-gnilcyceR
A1 A2 A3 A4 A5 B1 B2 B3 B4 B5 B6 B7 C1 C2 C3 C4 D
X X X X X X X X X X X X X X X X X
Product stage, A1-A3
Description of the stage:
The product stage of the mineral wool products is subdivided into 3 modules A1, A2 and A3
respectively “Raw material supply”, “transport” and “manufacturing”.
The aggregation of the modules A1, A2 and A3 is a possibility considered by the EN 15 804 standard.
This rule is applied in this EPD.
A1, Raw material supply
This module takes into account the extraction and processing of all raw materials and energy which
occur upstream to the studied manufacturing process.
Specifically, the raw material supply covers production of binder components and sourcing (quarry) of
raw materials for fiber production, e.g. sand and borax for glass wool. Besides these raw materials,
recycled material/glass cullet is also used as input.
About cullet: The main raw material for the production of glass insulation material is cullets or/and sand.
Only specific cleaning activities and transport is included for the cullets – and thus not the impacts from
the full life cycle of glass. The reason is that cullets are considered a waste product and not initially
produced for the purpose of glass wool insulation production. The only activities included are:
• Magnetic separation of metallic piece
• Separation of other piece-crushing of glass (<20 mm)
• Separation of bottle cap crushing (<2 mm) sieving
• Transport
A2, transport to the manufacturer
The raw materials are transported to the manufacturing site. In our case, the modeling includes: road
and boat transportations (specific values) of each raw material.
A3, manufacturing
This module covers glass wool fabrication, including melting and fiberization (see process flow
diagram). In addition, the production of packaging material is taking into account at this stage.
NEPD-2502-1244-EN ISOVER Fasadskiva 30 Alu
Manufacturing process flow diagram
Construction process stage, A4-A5
Description of the stage:
The construction process is divided into 2 modules: A4, transport to the building site and A5, installation
in the building.
Description of scenarios and additional technical information:
A4, Transport to the building site:
- This module includes transport from the production gate to the building site. (Representative as
average for the Swedish and Norwegian market).
- Transport is calculated on the basis of a scenario with the parameters described in the following
table.
PARAMETER VALUE (per functional unit)
Fuel type and consumption of vehicle or vehicle
Average truck trailer with a 27t payload, diesel
type used for transport e.g. long distance truck,
consumption 38 liters for 100 km
boat, etc.
Distance 500 km
77 % of the capacity in volume
Capacity utilisation (including empty returns) (40% capacity utilisation including 40 % of empty
returns in mass)
Bulk density of transported products 50 - 55 kg/m3
Volume capacity utilisation factor 1 (by default)
7
NEPD-2502-1244-EN ISOVER Fasadskiva 30 Alu
A5, Installation in the building:
This module includes:
- Wastage of products: see following table 5 %. These losses are landfilled (landfill model for glass
see chapter End of life),
- Additional production processes to compensate for the loss
- Processing of packaging wastes: they are 100 % collected and modeled as recovered matter.
This module does not include:
-Energy for installation of the insulation, as the installation is done manually, and do not require energy
PARAMETER VALUE (per functional unit)
Wastage of materials on the building site before
waste processing, generated by the product’s 5 %
installation (specified by type)
Distance 25 km to landfill by truck
Output materials (specified by type) as results of
Packaging wastes are 100 % collected and modeled
waste processing at the building site e.g. of
as recovered matter
collection for recycling, for energy recovering,
disposal
Glass wool losses are landfilled
(specified by route)
Use stage (excluding potential savings), B1-B7
Description of the stage: The use stage is divided into the following modules:
- B1: Use
- B2: Maintenance
- B3: Repair
- B4: Replacement
- B5: Refurbishment
- B6: Operational energy use
- B7: Operational water use
Description of scenarios and additional technical information:
Once installation is complete, no actions or technical operations are required during the use stages until
the end of life stage. Therefore, glass wool insulation products have no impact (excluding potential
energy savings) on this stage.
End-of-life stage C1-C4
Description of the stage: The stage includes the different modules of end-of-life detailed below.
C1, de-construction, demolition
The de-construction and/or dismantling of insulation products take part of the demolition of the entire
building and is assumed to be made manually. In our case, the environmental impact is assumed to be
very small and can be neglected.
C2, transport to waste processing
Transport is included and calculated on the basis of a scenario with the parameters described in the
End-of-life table.
C3, waste processing for reuse, recovery and/or recycling;
Today the product is considered to be landfilled without reuse, recovery or recycling.
C4, disposal;
The glass wool is assumed to be 100% landfilled.
8
NEPD-2502-1244-EN ISOVER Fasadskiva 30 Alu
Description of scenarios and additional technical information: See below
End-of-life:
PARAMETER VALUE (per functional unit)
The entire insulation product (wool and surfacing) is
collected with mixed construction waste
Collection process specified by type
1.74 kg of glass wool (collected with mixed
construction waste)
Recovery system specified by type No re-use, recycling or energy recovery
The entire insulation product (wool and surfacing) is
Disposal specified by type landfilled
1.74 kg of glass wool are landfilled
Average truck trailer with a 27t payload, diesel
consumption 38 liters for 100 km
Assumptions for scenario development (e.g.
transportation)
25 km (default distance from the building site to
landfill).
Reuse/recovery/recycling potential, D
Description of the stage: For module D we only take into consideration the materials used within
the product, and not e.g. packaging and that the benefit then will be equal to zero.
LCA results
LCA model, aggregation of data and potential environmental impact are calculated from the GaBi
software 8.7 and CML impact method has been used, together with thinkstep 8.7 (2018) and ecoinvent
V3.1 (2014) databases to obtain the inventory of generic data. Biogenic carbon is not reported in the
context of GWP.
Raw materials and energy consumption, as well as transport distances have been taken directly from
the manufacturing plant of Saint-Gobain Sweden A, ISOVER in Billesholm (Production data according
2018).
Resume of the LCA results detailed on the following tables.
9
NEPD-2502-1244-EN ISOVER Fasadskiva 30 Alu
ENVIRONMENTAL IMPACTS
Product Construction
Use stage End-of-life stage
stage process stage
Parameters
10
3A
/
2A
/
1A
tropsnarT
4A
noitallatsnI
5A
esU
1B
ecnanetniaM
2B
riapeR
3B
4B
tnemecalpeR
5B
tnemhsibrufeR lanoitarepO
6B
esu
ygrene
lanoitarepO
7B
esu
retaw 1C
/ noitcurtsnoceD noitilomed tropsnarT
2C
etsaW
3C
gnissecorp lasopsiD
4C
,yrevocer
,esueR
D
gnilcycer
2.53E+00 8,41E-02 1,38E-01 0 0 0 0 0 0 0 0 8,52E-03 0 1,01E-01 0
Global Warming Potential
(GWP) - kg CO2 equiv/FU
The global warming potential of a gas refers to the total contribution to global warming resulting from the emission
of one unit of that gas relative to one unit of the reference gas. carbon dioxide. which is assigned a value of 1.
2.16E-07 1,28E-17 1,08E-08 0 0 0 0 0 0 0 0 9,28E-15 0 1,79E-16 0
Ozone Depletion (ODP)
kg CFC 11 equiv/FU Destruction of the stratospheric ozone layer which shields the earth from ultraviolet radiation harmful to life.
This destruction of ozone is caused by the breakdown of certain chlorine and/or bromine containing compounds (chlorofluorocarbons or halons).
which break down when they reach the stratosphere and then catalytically destroy ozone molecules.
1.52E-02 3,58E-04 7,98E-04 0 0 0 0 0 0 0 0 3,48E-05 0 1,85E-04 0
Acidification potential (AP)
kg SO2 equiv/FU
Acid depositions have negative impacts on natural ecosystems and the man-made environment incl. buildings.
The main sources for emissions of acidifying substances are agriculture and fossil fuel combustion used for electricity production. heating and transport.
Eutrophication potential (EP) 5.61E-03 8,79E-05 2,93E-04 0 0 0 0 0 0 0 0 8,39E-06 0 1,17E-04 0
kg (PO4)3- equiv/FU
Excessive enrichment of waters and continental surfaces with nutrients. and the associated adverse biological effects.
Photochemical ozone 1.37E-03 1,31E-05 7,13E-05 0 0 0 0 0 0 0 0 1,30E-06 0 3,60E-05 0
creation (POPC)
kg Ethene equiv/FU Chemical reactions brought about by the light energy of the sun.
The reaction of nitrogen oxides with hydrocarbons in the presence of sunlight to form ozone is an example of a photochemical reaction.
Abiotic depletion potential for
non-fossil ressources (ADP- 1.54E-04 1,12E-09 7,69E-06 0 0 0 0 0 0 0 0 1,16E-10 0 1,07E-08 0
elements) - kg Sb equiv/FU
Abiotic depletion potential for
3.91E+01 1,17E+00 2,06E+00 0 0 0 0 0 0 0 0 1,19E-01 0 4,91E-01 0
fossil ressources (ADP-fossil
fuels) - MJ/FU
Consumption of non-renewable resources. thereby lowering their availability for future generations.
NEPD-2502-1244-EN ISOVER Fasadskiva 30 Alu
RESOURCE USE
Product Construction
Use stage End-of-life stage
stage process stage
Parameters
11
3A
/
2A
/
1A
tropsnarT
4A
noitallatsnI
5A
esU
1B
ecnanetniaM
2B
riapeR
3B
4B
tnemecalpeR
5B
tnemhsibrufeR lanoitarepO
6B
esu
ygrene
lanoitarepO
7B
esu
retaw 1C
/ noitcurtsnoceD noitilomed tropsnarT
2C
etsaW
3C
gnissecorp lasopsiD
4C
.yrevocer
.esueR
D
gnilcycer
Use of renewable primary
energy excluding renewable
3.94E+01 2.7E-02 2.0E+00 0 0 0 0 0 0 0 0 3.2E-03 0 5.6E-02 0
primary energy resources used
as raw materials - MJ/FU
Use of renewable primary
energy used as raw materials 4.05E+00 0 2.0E-01 0 0 0 0 0 0 0 0 0 0 0 0
MJ/FU
Total use of renewable primary energy
resources (primary energy and
4.35E+01 2.7E-02 2.2E+00 0 0 0 0 0 0 0 0 3.2E-03 0 5.6E-02 0
primary energy resources used as raw
materials) MJ/FU
Use of non-renewable primary
energy excluding non-renewable
4.25E+01 1.2E+00 2.2E+00 0 0 0 0 0 0 0 0 1.2E-01 0 5.1E-01 0
primary energy resources used
as raw materials - MJ/FU
Use of non-renewable primary
energy used as raw materials 3.24E+00 0 1.6E-01 0 0 0 0 0 0 0 0 0 0 0 0
MJ/FU
Total use of non-renewable primary
energy resources (primary energy and
4.57E+01 1.2E+00 2.4E+00 0 0 0 0 0 0 0 0 1.2E-01 0 5.1E-01 0
primary energy resources used as raw
materials) - MJ/FU
Use of secondary material
9.96E-01 0 5.0E-02 0 0 0 0 0 0 0 0 0 0 0 0
kg/FU
Use of renewable secondary
0 0 0 0 0 0 0 0 0 0 0 0 0 0 0
fuels- MJ/FU
Use of non-renewable
0 0 0 0 0 0 0 0 0 0 0 0 0 0 0
secondary fuels - MJ/FU
Use of net fresh water - m3/FU 4.94E-02 9.0E-06 2.5E-03 0 0 0 0 0 0 0 0 1.0E-06 0 1.1E-04 0
NEPD-2502-1244-EN ISOVER Fasadskiva 30 Alu
WASTE CATEGORIES
Product Construction
Use stage End-of-life stage
stage process stage
Parameters
12
3A
/
2A
/
1A
tropsnarT
4A
noitallatsnI
5A
esU
1B
ecnanetniaM
2B
riapeR
3B
4B
tnemecalpeR
5B
tnemhsibrufeR lanoitarepO
6B
esu
ygrene
lanoitarepO
7B
esu
retaw 1C
/ noitcurtsnoceD noitilomed tropsnarT
2C
etsaW
3C
gnissecorp lasopsiD
4C
.yrevocer
.esueR
D
gnilcycer
Hazardous waste disposed
7.73E-08 4.21E-09 4.56E-09 0 0 0 0 0 0 0 0 4.27E-10 0 6.88E-09 0
kg/FU
Non-hazardous waste disposed
kg/FU
2.01E-01 1.42E-05 1.15E-01 0 0 0 0 0 0 0 0 1.61E-06 0 1.83E+00 0
Radioactive waste disposed
6.77E-04 1.37E-06 3.44E-05 0 0 0 0 0 0 0 0 1.39E-07 0 6.73E-06 0
kg/FU
NEPD-2502-1244-EN ISOVER Fasadskiva 30 Alu
OUTPUT FLOWS
Product Construction
Use stage End-of-life stage
stage process stage
Parameters
13
3A
/
2A
/
1A
tropsnarT
4A
noitallatsnI
5A
esU
1B
ecnanetniaM
2B
riapeR
3B
4B
tnemecalpeR
5B
tnemhsibrufeR lanoitarepO
6B
esu
ygrene
lanoitarepO
7B
esu
retaw 1C
/ noitcurtsnoceD noitilomed tropsnarT
2C
etsaW
3C
gnissecorp lasopsiD
4C
.yrevocer
.esueR
D
gnilcycer
Components for re-use
0 0 0 0 0 0 0 0 0 0 0 0 0 0 0
kg/FU
Materials for recycling
kg/FU
2.98E-02 0 2.70E-01 0 0 0 0 0 0 0 0 0 0 0 0
Materials for energy recovery
0 0 0 0 0 0 0 0 0 0 0 0 0 0 0
kg/FU
Exported energy
0 0 0 0 0 0 0 0 0 0 0 0 0 0 0
MJ/FU
NEPD-2502-1244-EN ISOVER Fasadskiva 30 Alu
Product Transport Installation Use End-of-life
(A1-A3) (A4) (A5) (B) (C) Total Recycling
Environmental Positive benefits
impacts of the of recycling
product (D)
Global warming 3,00 2,53
2,00 2,86
1,00
0,08 0,14 0,00 0,11 0,00
0,00
Non-renewable resources 60,00
consumption [1] 39,10
40,00 42,94
20,00
1,17 2,06 0,00 0,61 0,00
0,00
Energy consumption [2] 100,00 89,20
95,66
50,00
1,20 4,58 0,00 0,69 0,00
0,00
Water consumption [3] 0,06 0,0494
0,04 0,05
0,02
0,0000 0,0025 0,0000 0,0001 0,0000
0,00
Waste production [4] 2,00 1,83
1,50
2,15
1,00
0,50 0,20 0,00 0,12 0,00 0,00
0,00
[1] This indicator corresponds to the abiotic depletion potential of fossil resources.
[2] This indicator corresponds to the total use of primary energy.
[3] This indicator corresponds to the use of net fresh water.
[4] This indicator corresponds to the sum of hazardous, non-hazardous and radioactive waste disposed.
Global Warming Potential (Climate Change) (GWP)
When analyzing the above figure for GWP. it can clearly be seen that the majority of contribution to this
environmental impact is from the production modules (A1-A3). This is primarily because the sources of
greenhouse gas emissions are predominant in this part of the life cycle. CO2 is generated upstream from the
production of electricity and is also released on site by the combustion of natural gas. We can see that other
sections of the life cycle also contribute to the GWP; however. the production modules contribute to over 80%
of the contribution. Combustion of fuel in transport vehicles will generate the second highest percentage of
greenhouse gas emissions together the waste during the installation stage.
Global warming potential does not account for emission and uptake of biogenic CO .
2
Non-renewable resources consumptions
We can see that the consumption of non – renewable resources is once more found to have the highest value
in the production modules. This is because a large quantity of natural gas is consumed within the factory. and
non – renewable fuels such as natural gas and coal are used to generate the large amount of electricity we
use. The contribution to this impact from the other modules is very small and primarily due to the non –
renewable resources consumed during transportation.
Energy Consumptions
As we can see. modules A1-A3 have the highest contribution to total energy consumption. Energy in the form
of electricity and natural gas is consumed in a vast quantity during the manufacture of glass mineral wool so
we would expect the production modules to contribute the most to this impact category.
14
UF/viuqe2OC
gk
UF/JM
UF/JM
UF/3m
UF/gk
LCA interpretation
kg CO2equiv/FU
MJ/FU
MJ/FU
m3/FU
kg/FU
NEPD-2502-1244-EN ISOVER Fasadskiva 30 Alu
Water Consumption
As we don’t use water in any of the other modules (A4-A5. B1-B7. C1-C4). we can see that there is no
contribution to water consumption. For the production phase. water is used within the manufacturing facility
and therefore we see the highest contribution here. However. we recycle a lot of the water on site so the
contribution is still relatively low.
Waste Production
Waste production does not follow the same trend as the above environmental impacts. The largest contributor
is the end of life module. This is because the entire product is sent to landfill once it reaches the end of life
state. However. there is still an impact associated with the production module since we do generate waste on
site. The following small impact associated with installation is due to the loss rate of product during
implementation.
Additional information
Influence of particular thicknesses
All the results in the table of this EPD refer to ISOVER Fasadskiva 30 Alu with a thickness of 30 mm for a
functional unit of 1 m² with a thermal resistance equals to 1.00 m² K/W
This EPD of ISOVER products mentioned above includes a range of thicknesses between 30 mm and 100
mm. For every thickness, use a multiplication factor in order to obtain the environmental performance of every
thickness. In order to calculate the multiplication factors, a reference unit has been selected R=1
The various multiplication factors are obtained by making the LCA calculations for all thicknesses. including
packaging. The GWP value in each thickness is chosen as a reference indicator to obtain the multiplication
factor. Using the thickness factor will for some indicators give higher values than calculated for the specific
thickness in GaBi.
In the table below the multiplication factors are shown for products and specific thickness of the product family.
In order to obtain the environmental performance associated with every specific product and thickness. the
results expressed in this EPD must be multiplied by its corresponding multiplication factor.
PRODUCT THICKNESS THERMAL
MULTIPLICATION FACTOR
(mm) RESISTANCE
30 1.00 1.00
50 1.67 1.47
80 2.67 2.16
100 3.33 2.63
15
NEPD-2502-1244-EN ISOVER Fasadskiva 30 Alu
Additional Norwegian requirements
Greenhouse gas emissions from the use of electricity in the manufacturing phase
The LCA calculation has been made taking into account the fact that during the manufacturing process it is
used 100% renewable electricity. This 100% renewable electricity bought is evidenced by Guarantee of Origin
certificates. GO’s. from LOS. contracted 2018- 2020. to be prolonged to be valid at least equal to the validity
of this EPD
TYPE OF INFORMATION DESCRIPTION
Location Representative of average production in Sweden
Split of energy sources in Sweden
Geographical representativeness description -Hydro: 54%
-Biomass: 46%
Reference year 2018
Type of data set Cradle to gate from Thinkstep
Gabi database from International Energy Agency -2013
Source
Guarantee of Origin certificates (GOs) - 2018
Electricity Mix (from renewable sources) -
Sweden
46% Biomass
54% Hydro
The dataset used to model the renewable electricity mix used for these calculations come from thinkstep
database.
DATA SOURCE AMOUNT UNIT
thinkstep (2018) 0.05 kg CO2 eq /KWh
Dangerous substances
The product contains no substances given by the REACH Candidate list (of 15.01.2018) or the Norwegian
priority list. (REACH registration number 01-2119472313-44-0039)
Indoor environment
No test performed
Carbon footprint
Carbon footprint has not been worked out for the product
16
NEPD-2502-1244-EN ISOVER Fasadskiva 30 Alu
Bibliography
- Product-Category Rules. NPCR 012:2018 Part B for Thermal insulation products
- Environmental labels and declarations - Type III environmental declarations -Principles and procedures
(ISO 14025:2006)
- Environmental management - Life cycle assessment – Requirements and guidelines (ISO 14044:2006)
- Sustainability of construction works - Environmental product declaration - Core rules for the product
category of construction products (EN 15804:2012+2013:A1)
- Sustainability in building construction - Environmental declaration of building products (ISO 21930:2017)
- Ecoinvent database V3.1 (2014)
- Gabi 8.7 database (2018)
- SS-EN 13172:2012 Thermal Insulation Products – Evaluation of conformity
- SS- EN 14303 “Thermal insulation products for building equipment and industrial installations. Factory
made mineral wool (MW) products. Specification
- LCA report. Information for the Environmental Product Declaration of Isover product. Saint-Gobain
Sweden AB Isover. November 2019, rev. September 2020
Program operator and Publisher Phone: +47 23 08 80 00
The Norwegian EPD Foundation
Post Box 5250 Majorstuen. 0303 Oslo e-mail: post@epd-
Norway web norge.no
www.epd-
norge.no
Owner of the declaration Phone: +46 (0)42-842 52
Saint-Gobain Sweden AB e-mail: daniel.odby@saint-
gobain.com
Company logo web www.isover.se
Author of the Life Cycle Assessment Phone: +33 1 47 62 42 65
Patricia Jimenez Diaz e-mail: Patricia.jimenezdiaz@
Saint-Gobain. Central Marketing & Development saint-gobain.com
<xxxx>
17
NEPD-2502-1244-EN ISOVER Fasadskiva 30 Alu
