ENVIRONMENTAL PRODUCT DECLARATION
as per ISO 14025 and EN 15804+A2
Owner of the Declaration JANSEN AG
Publisher Institut Bauen und Umwelt e.V. (IBU)
Programme holder Institut Bauen und Umwelt e.V. (IBU)
Declaration number EPD-JAN-20240300-CBA1-EN
Issue date 29.11.2024
Valid to 28.11.2029
Janisol Primo window width x height: 1230 mm x 1480 mm
Jansen AG
www.ibu-epd.com | https://epd-online.com
General Information
Jansen AG Janisol Primo window width x height: 1230 mm x
1480 mm
Programme holder Owner of the declaration
IBU – Institut Bauen und Umwelt e.V. JANSEN AG
Hegelplatz 1 Industriestrasse 34
10117 Berlin 9463 Oberriet
Germany Switzerland
Declaration number Declared product / declared unit
EPD-JAN-20240300-CBA1-EN 1 m2 Janisol Primo window with a grammage of 42.24 kg/m². The actual
reference size of the declared window has dimensions of width x height:
1230 mm x 1480 mm.
This declaration is based on the product category rules: Scope:
Windows and doors , 01.08.2021 The environmental product declaration refers to a window type Janisol
(PCR checked and approved by the SVR) Primo in specific dimension width x height. The characteristic values used
for the system components Janisol Primo in the LCA are provided by
Jansen AG.
Issue date
The declared product is defined according to the profile series and product
29.11.2024
characteristics.
The location of the production site is Oberriet/Switzerland.
Valid to
This EPD was created with the help of a semi-automatic LCA-Tool.
28.11.2029 The owner of the declaration shall be liable for the underlying information
and evidence; the IBU shall not be liable with respect to manufacturer
information, life cycle assessment data and evidences.
The EPD was created according to the specifications of EN 15804+A2. In
the following, the standard will be simplified as EN 15804.
Verification
The standard EN 15804 serves as the core PCR
Independent verification of the declaration and data according to ISO
14025:2011
Dipl.-Ing. Hans Peters internally X externally
(Chairman of Institut Bauen und Umwelt e.V.)
Florian Pronold Matthias Schulz,
(Managing Director Institut Bauen und Umwelt e.V.) (Independent verifier)
1 Environmental Product Declaration - Jansen AG - Janisol Primo window width x height: 1230 mm x 1480 mm
Product
Constructional data
Product description/Product definition
Janisol Primo windows are made of steel profiles with a depth Name Value Unit
of 60 mm and a slender face width. The processing of Janisol Resistance to wind load acc. to EN
C4 class
Primo and the combination with Janisol systems is made 12210
simpler by identical profile shapes and produces better Water tightness acc. to EN 12208 9A class
insulation values. This declaration describes the following
Sound insulation class acc. to EN up to Rw 45 dB
element in Janisol Primo: -
EN ISO 10140 (-2; -5)
Product: Janisol Primo
Heat transfer coefficient acc. to DIN
Width x height: 1230 mm x 1480 mm 1.5 W/(m2K)
EN ISO 10077-2
Face width sash: 82.5 mm / transom 103 mm
Basic depth: 60 mm / sash depth: 64 mm Air permeability acc. to EN 12207 4 class
CE marking according to EN 14351-1 Mechanical strength acc. to EN
1 class
13115
The products require a declaration of performance taking into Bullet proofing acc. to EN 1522 FB4-FB6 class
account the harmonized product standard EN 14351-1 windows Burglar resistance acc. to EN 1627 RC1-RC3 class
and doors and a CE marking. The respective national
regulations apply to the use. With this declaration the following Product according to the CPR, based on EN: Performance data
element is declared: of the product in accordance with the declaration of
performance with respect to its essential characteristics
according to EN 14351-1, windows. Other constructional data
are not relevant for this product.
Base materials/Ancillary materials
JANSEN Janisol Primo window is made of the following
materials:
• Glazing approx. 38%
• Steel approx. 49%
• Plastics and fillers approx. 7%
• Fittings approx. 4%
• Aluminium 2%
The percentages relate to the most frequently sold product with
an opening of 1.82 m2. The percentages stated may vary
depending on the product type and dimensions.
Does the product or at least one part product contain materials
from the ECHA candidate list of materials which are especially
problematic for approval: Substances of Very High Concern –
SVHC (date 27.06.2024) above a mass % of 0.1: no.
This product/article/at least one partial article contains other
CMR substances in categories 1A or 1B which are not on the
candidate list, exceeding 0.1 percentage by mass: no.
Biocide products were added to this construction product or it
has been treated with biocide products (this then concerns a
treated product as defined by the (EU) Ordinance on Biocide
Products No. 528/2012): no.
Reference service life
According to SBR 2011 regarding the specific material
Application
characteristics of steel windows and doors, the reference
The Janisol Primo opening element can be integrated for
service life is 75 years (SBR 2011). The practical service life
building ventilation and light transmission.
may well be longer. Conditions for a long service life are regular
maintenance, care and upkeep of the product. The specified
Technical Data
service life is independent of the manufacturer's warranty.
According to the CE marking, the following structural data for
the element must be stated:
LCA: Calculation rules
Declared unit
Declared Unit
The declared unit is a 1 m2 of Janisol Primo window element. Name Value Unit
Declared unit 1 m2
The actual reference size of the declared window element has Grammage 42.24 kg/m2
dimensions of 1230 mm x 1480 mm.
Layer thickness 0.06 m
2 Environmental Product Declaration - Jansen AG - Janisol Primo window width x height: 1230 mm x 1480 mm
Other declared units are allowed if the conversion is shown Scenario 0: 100% thermal treatment of all raw materials with
transparently. heating value including plastic system parts and 100%
recycling of metal system components (C3). Landfill of all
For inhomogeneous components made of different materials, materials without heating value (except metals) including
the conversion to other dimensions with factors leads to glazing (C4).
deviations compared to the exact calculation. The frame Scenario 1 (module C3/1): 100% recycling of plastic system
percentage is 23.82% and the ground reference is 0.074m². parts and 100% recycling of metal system components. Landfill
of all materials without heating value (except metals) including
frame percentage = frame surface / total area x 100 [%] glazing (C4/1).
ground reference = element depth x element width [m²] Modules C4 & C4/1 are identical.
System boundary
EoL scenario 0 (modules C3 and C4)
Type of EPD according to EN 15804: "cradle to gate with Collected separately waste type (window element) 42.24 kg
options, modules C1–C4, and module D". The following Recycling (C3) 22.83 kg
modules are declared: A1–A3, C, D and additional modules: A4 Energy recovery (C3) 3.49 kg
+ A5. Landfilling (C4) 16.05 kg
Production (modules A1-A3): EoL scenario 1 (modules C3/1 and C4/1)
Collected separately (window element) 42.24 kg
This module considers the provision of all relevant window Recycling (C3/1) 26.16 kg
components (i.e. metal profiles/ components, glass units and Energy recovery (C3/1) 0.16 kg
plastic parts/profiles) and raw materials including their transport Landfilling (C4/1) 16.05 kg
to the declared production plant. This considers the
manufacturing and assembly of these components, including
waste processing up to the end-of-waste state. The impact of Benefits and loads beyond the product system boundary
packaging materials is also covered by this module. (module D):
Transport to the construction site (module A4): Considers credits and loads from the recycling of the metal
components (duplicated in D and D/1) and the recycling of the
A distance of 100 km is considered for the transport of the plastic system parts/profiles (D/1). Avoided burdens from the
packed finished product via truck. The transport distance can thermal treatment of all raw materials with heating value
be modified project-specific if required by linear scaling. (including plastic system parts/ profiles) (D) and packaging
treatment (duplicated in D and D/1) under European conditions
Installation (module A5): are considered. This affects only the rate of primary materials
(no secondary materials).
Treatment and disposal of packaging material is considered in
this module. Credits for potential avoided burdens due to Geographic Representativeness
energy substitution of electricity and thermal energy generation Land or region, in which the declared product system is
are declared in module D under European conditions and manufactured, used or handled at the end of the product´s
affects only the rate of primary materials (no secondary lifespan: Europe
materials).
Comparability
EoL stage (modules C1-C4):
Basically, a comparison or an evaluation of EPD data is only
Module C1 - considers manual deconstruction (without possible if all the data sets to be compared were created
environmental burdens). according to EN 15804 and the building context, respectively
Module C2 - considers 50 km truck transport to waste the product-specific characteristics of performance, are taken
processing. The transport distance can be modified project- into account. The following background database has been
specific if required by linear scaling. used for the LCA calculation: Sphera LCA software (GaBi ts)
Modules C3 and C4 - consider waste processing and/or content update package (CUP) version 2022.2
disposal with the following scenarios:
LCA: Scenarios and additional technical information
Characteristic product properties of biogenic carbon The following technical information is a basis for the declared
No biogenic carbon is reported in the product. The biogenic modules. The values refer to the declared unit of 1 m2 of
carbon content in the accompanying packaging for 1 m2 Janisol Janisol Primo window.
Primo window is declared below.
Transport to the building site (A4)
Information on describing the biogenic Carbon Content at
Name Value Unit
factory gate
Litres of fuel 0.0832 l/100km
Name Value Unit
Transport distance 100 km
kg
Biogenic carbon content in product - Capacity utilisation (including empty runs) 61 %
C
Gross weight of packed products transported 42.26 kg
Biogenic carbon content in accompanying kg
0.01168
packaging C
Installation into the building (A5)
Note: 1kg of biogenic carbon is equivalent to 44/12 kg of CO2.
3 Environmental Product Declaration - Jansen AG - Janisol Primo window width x height: 1230 mm x 1480 mm
Name Value Unit EPD is currently considered a scenario that is not widely
available in reality due to economic viability limitations
Polyethylene (waste packaging to incineration) 0.00252 kg
associated with higher costs of sorting smaller shares of
Cardboard box (waste packaging to incineration) 0.01204 kg
plastics such as those present in the declared product.
Wood (waste packaging to incineration) 0.01588 kg
Name ValueUnit
According to SBR 2011 regarding the specific material
EoL scenario 0 (modules C3 and C4)
characteristics of steel windows and doors, the reference
Collected separately waste type (window element) 42.24 kg
service life is 75 years (SBR 2011). The practical service life
Recycling (C3) 22.83 kg
may well be longer. Conditions for a long service life are regular
maintenance, care and upkeep of the product. The specified Energy recovery (C3) 3.49 kg
service life is independent of the manufacturer's warranty. Landfilling (C4) 16.05 kg
EoL scenario 1 (modules C3/1 and C4/1)
Collected separately (window element) 42.24 kg
Reference service life Recycling (C3/1) 26.16 kg
Energy recovery (C3/1) 0.16 kg
Name Value Unit Landfilling (C4/1) 16.05 kg
Life Span (according to SBR 2011) 75 a
Reuse, recovery and/or recycling potentials (D), relevant
Reference service life according to SBR 2011. scenario information
End of life (C1-C4) Module D includes the credits and loads from the recycling of
the metal components (duplicated in D and D/1) and the
For the End-of-Life stage two scenarios are considered.
recycling of the plastic system parts/profiles (D/1). Avoided
Scenario 0 considers 100% thermal treatment of all raw
burdens from the thermal treatment of all raw materials with
materials with heating value including plastic system parts and
heating value (including plastic system parts/profiles) (D) and
100% recycling of metal system components (C3). Landfill of all
packaging treatment (duplicated in D and D/1) under European
materials without heating value (except metals) including
conditions are considered. This affects only the rate of primary
glazing (C4). Scenario 1 considers 100% recycling of plastic
materials (no secondary materials). A waste incineration plant
system parts and 100% recycling of metal system components
with R1-value > 0.6 is assumed.
(C3/1). Landfill of all materials without heating value (except
metals) including glazing (C4/1). Modules C4 and C4/1 are
For recycling, a collection rate of 100% is considered.
identical. The recycling of plastics scenario declared in this
4 Environmental Product Declaration - Jansen AG - Janisol Primo window width x height: 1230 mm x 1480 mm
LCA: Results
Results provided in this section are presented in relation to 1 m2 of window type Jansen Janisol Primo (reference dimensions 1230 mm
x 1480 mm).
For the End-of-Life stage, two scenarios are considered:
C3 - considers 100% recycling of metal system components (duplicated in D and D/1) and 100% thermal treatment of all raw materials
with heating value including plastic system parts.
C3/1 - considers 100% recycling of metal system components (duplicated in D and D/1) and 100% recycling of plastic system parts.
C4 and C4/1 - considers landfill of all materials without heating value (except metals) including glazing. Modules C4 and C4/1 are
identical.
D - considers credits and loads from the recycling of the metal components (duplicated in D and D/1). Avoided burdens from packaging
treatment (duplicated in D and D/1) and thermal treatment of all raw materials with heating value (including plastic system
parts/profiles) are considered.
D/1 - considers credits and loads from the recycling of the metal components (duplicated in D and D/1) and the recycling of the plastic
system parts/profiles. Avoided burdens from packaging treatment (duplicated in D and D/1) are considered.
DESCRIPTION OF THE SYSTEM BOUNDARY (X = INCLUDED IN LCA; MND = MODULE OR INDICATOR NOT DECLARED; MNR
= MODULE NOT RELEVANT)
Benefits and
Construction loads beyond
Product stage Use stage End of life stage
process stage the system
boundaries
la ire ta m w a Ry lp p u s tro p s n a rT g n iru tc a fu n a M e h t m o rf tro p s n a rTe tis e h t o t e ta g y lb m e s s A e s U e c n a n e tn ia M ria p e R tn e m e c a lp e R tn e m h s ib ru fe R y g re n e la n o ita re p Oe s u re ta w la n o ita re p Oe s u n o itc u rts n o c -e Dn o itilo m e d tro p s n a rT g n is s e c o rp e ts a W la s o p s iD -e s u e R-y re v o c e R-g n ilc y c e Rla itn e to p
A1 A2 A3 A4 A5 B1 B2 B3 B4 B5 B6 B7 C1 C2 C3 C4 D
X X X X X MND MND MNR MNR MNR X MND X X X X X
RESULTS OF THE LCA - ENVIRONMENTAL IMPACT according to EN 15804+A2: 1 m2 Janisol Primo window (42.24 kg/m2)
Parameter Unit A1-A3 A4 A5 B6 C1 C2 C3 C3/1 C4 C4/1 D D/1
GWP-total kg CO 2 eq 7.83E+01 2.55E-01 5.11E-02 0 0 1.27E-01 8.2E+00 1.26E-01 2.41E-01 2.41E-01 -2.39E+01 -2.31E+01
GWP-fossil kg CO 2 eq 7.81E+01 2.53E-01 8.7E-03 0 0 1.26E-01 8.2E+00 1.26E-01 2.39E-01 2.39E-01 -2.38E+01 -2.31E+01
GWP-
biogenic kg CO 2 eq 2.49E-01 1.07E-03 4.24E-02 0 0 5.33E-04 6.12E-04 3.18E-05 8.06E-04 8.06E-04 -1.69E-02 -2.13E-02
GWP-luluc kg CO 2 eq 2.38E-02 1.41E-03 1.39E-07 0 0 7.05E-04 6.42E-05 5.05E-06 4.42E-04 4.42E-04 -1.08E-03 -1.65E-03
kg CFC11
ODP 4.04E-10 1.52E-14 4.39E-15 0 0 7.58E-15 1.2E-12 4.64E-14 5.63E-13 5.63E-13 -2.04E-11 -1.27E-10
eq
AP mol H+ eq 2.5E-01 2.41E-04 9.56E-06 0 0 1.2E-04 2.18E-03 3.13E-05 1.7E-03 1.7E-03 -5.88E-02 -6.06E-02
EP-
kg P eq 8.36E-05 7.55E-07 1.19E-09 0 0 3.77E-07 3.67E-07 3.46E-08 4.06E-07 4.06E-07 -8.39E-06 -1.27E-05
freshwater
EP-marine kg N eq 7.39E-02 7.5E-05 3.21E-06 0 0 3.75E-05 7.57E-04 1.1E-05 4.34E-04 4.34E-04 -9.5E-03 -1E-02
EP-terrestrial mol N eq 8.5E-01 9.01E-04 4.44E-05 0 0 4.5E-04 1.08E-02 1.51E-04 4.77E-03 4.77E-03 -8.95E-02 -9.43E-02
kg NMVOC
POCP 2.15E-01 2.1E-04 8.63E-06 0 0 1.05E-04 1.99E-03 2.96E-05 1.32E-03 1.32E-03 -3.55E-02 -4.06E-02
eq
ADPE kg Sb eq 1.6E-04 2.11E-08 1.07E-10 0 0 1.06E-08 2.96E-08 1.08E-09 2.45E-08 2.45E-08 -4.35E-05 -4.38E-05
ADPF MJ 9.86E+02 3.38E+00 1.21E-02 0 0 1.69E+00 2.36E+00 8.59E-02 3.14E+00 3.14E+00 -2.55E+02 -3.12E+02
m3 world eq
WDP 5.32E+00 2.27E-03 5.82E-03 0 0 1.13E-03 7.9E-01 2.55E-02 2.63E-02 2.63E-02 -4.05E+00 -4.46E+00
deprived
GWP = Global warming potential; ODP = Depletion potential of the stratospheric ozone layer; AP = Acidification potential of land and water; EP =
Eutrophication potential; POCP = Formation potential of tropospheric ozone photochemical oxidants; ADPE = Abiotic depletion potential for non-fossil
resources; ADPF = Abiotic depletion potential for fossil resources; WDP = Water (user) deprivation potential)
RESULTS OF THE LCA - INDICATORS TO DESCRIBE RESOURCE USE according to EN 15804+A2: 1 m2 Janisol Primo window
(42.24 kg/m2)
Parameter Unit A1-A3 A4 A5 B6 C1 C2 C3 C3/1 C4 C4/1 D D/1
PERE MJ 1.24E+02 1.92E-01 4.23E-01 0 0 9.61E-02 6.08E-01 2.81E-02 4.71E-01 4.71E-01 -2.67E+01 -1.6E+01
PERM MJ 4.2E-01 0 -4.2E-01 0 0 0 0 0 0 0 0 0
PERT MJ 1.24E+02 1.92E-01 2.77E-03 0 0 9.61E-02 6.08E-01 2.81E-02 4.71E-01 4.71E-01 -2.67E+01 -1.6E+01
PENRE MJ 8.86E+02 3.39E+00 1.28E-01 0 0 1.69E+00 1.05E+02 1.02E+02 3.14E+00 3.14E+00 -2.55E+02 -3.12E+02
PENRM MJ 1.02E+02 0 -1.16E-01 0 0 0 -1.02E+02 -1.02E+02 0 0 0 0
PENRT MJ 9.88E+02 3.39E+00 1.21E-02 0 0 1.69E+00 2.37E+00 8.59E-02 3.14E+00 3.14E+00 -2.55E+02 -3.12E+02
SM kg 1.3E+01 0 0 0 0 0 0 0 0 0 1.04E+01 1.21E+01
RSF MJ 0 0 0 0 0 0 0 0 0 0 0 0
NRSF MJ 0 0 0 0 0 0 0 0 0 0 0 0
FW m3 2.39E-01 2.17E-04 1.37E-04 0 0 1.09E-04 1.86E-02 5.75E-04 7.97E-04 7.97E-04 -1.43E-01 -1.49E-01
5 Environmental Product Declaration - Jansen AG - Janisol Primo window width x height: 1230 mm x 1480 mm
PERE = Use of renewable primary energy excluding renewable primary energy resources used as raw materials; PERM = Use of renewable primary
energy resources used as raw materials; PERT = Total use of renewable primary energy resources; PENRE = Use of non-renewable primary energy
excluding non-renewable primary energy resources used as raw materials; PENRM = Use of non-renewable primary energy resources used as raw
materials; PENRT = Total use of non-renewable primary energy resources; SM = Use of secondary material; RSF = Use of renewable secondary fuels;
NRSF = Use of non-renewable secondary fuels; FW = Use of net fresh water
RESULTS OF THE LCA – WASTE CATEGORIES AND OUTPUT FLOWS according to EN 15804+A2:
1 m2 Janisol Primo window (42.24 kg/m2)
Parameter Unit A1-A3 A4 A5 B6 C1 C2 C3 C3/1 C4 C4/1 D D/1
HWD kg 1.95E-06 1.62E-11 1.18E-12 0 0 8.11E-12 2.33E-10 5.56E-12 1.61E-10 1.61E-10 4.51E-09 -9.52E-07
NHWD kg 3.12E+00 4.85E-04 7.73E-04 0 0 2.43E-04 3.95E-01 1.57E-02 1.61E+01 1.61E+01 1.32E+00 1.4E+00
RWD kg 2.7E-02 4.17E-06 6.88E-07 0 0 2.09E-06 8.68E-05 6.03E-06 3.5E-05 3.5E-05 -6.78E-03 -3.52E-03
CRU kg 0 0 0 0 0 0 0 0 0 0 0 0
MFR kg 6.17E-01 0 0 0 0 0 2.28E+01 2.62E+01 0 0 0 0
MER kg 0 0 0 0 0 0 0 0 0 0 0 0
EEE MJ 0 0 5.84E-02 0 0 0 1.31E+01 1.39E-01 0 0 0 0
EET MJ 0 0 1.05E-01 0 0 0 2.73E+01 2.89E-01 0 0 0 0
HWD = Hazardous waste disposed; NHWD = Non-hazardous waste disposed; RWD = Radioactive waste disposed; CRU = Components for re-use;
MFR = Materials for recycling; MER = Materials for energy recovery; EEE = Exported electrical energy; EET = Exported thermal energy
RESULTS OF THE LCA – additional impact categories according to EN 15804+A2-optional:
1 m2 Janisol Primo window (42.24 kg/m2)
Parameter Unit A1-A3 A4 A5 B6 C1 C2 C3 C3/1 C4 C4/1 D D/1
Disease
PM 2.28E-06 1.46E-09 5.03E-11 0 0 7.28E-10 1.39E-08 7.73E-10 2.09E-08 2.09E-08 -7.38E-07 -7.52E-07
incidence
kBq U235
IR 4.37E+00 6.11E-04 1.12E-04 0 0 3.06E-04 1.08E-02 7.24E-04 3.88E-03 3.88E-03 -8.91E-01 -3.31E-01
eq
ETP-fw CTUe 1.26E+03 2.35E+00 5.54E-03 0 0 1.17E+00 1.25E+00 6.29E-02 1.76E+00 1.76E+00 -3.66E+01 -8.14E+01
HTP-c CTUh 4.98E-08 4.73E-11 3.64E-13 0 0 2.36E-11 8.67E-11 2E-12 2.68E-10 2.68E-10 -9.51E-09 -1.05E-08
HTP-nc CTUh 1.1E-06 2.45E-09 1.37E-11 0 0 1.22E-09 5.77E-09 7.6E-11 2.97E-08 2.97E-08 -2.93E-07 -3.3E-07
SQP SQP 9.12E+01 1.16E+00 3.5E-03 0 0 5.81E-01 6.32E-01 3.04E-02 6.53E-01 6.53E-01 -7.98E+00 -1.11E+00
PM = Potential incidence of disease due to PM emissions; IR = Potential Human exposure efficiency relative to U235; ETP-fw = Potential comparative
Toxic Unit for ecosystems; HTP-c = Potential comparative Toxic Unit for humans (cancerogenic); HTP-nc = Potential comparative Toxic Unit for humans
(not cancerogenic); SQP = Potential soil quality index
Disclaimer 1 – for the indicator 'Potential Human exposure efficiency relative to U235'.This impact category deals mainly with the
eventual impact of low dose ionizing radiation on human health of the nuclear fuel cycle. It does not consider effects due to possible
nuclear accidents, occupational exposure nor due to radioactive waste disposal in underground facilities. Potential ionizing radiation
from the soil, from radon and from some construction materials is also not measured by this indicator.
Disclaimer 2 – for the indicators 'abiotic depletion potential for non-fossil resources', 'abiotic depletion potential for fossil resources',
'water (user) deprivation potential, deprivation-weighted water consumption', 'potential comparative toxic unit for ecosystems', 'potential
comparative toxic unit for humans – cancerogenic', 'Potential comparative toxic unit for humans - not cancerogenic', 'potential soil
quality index'. The results of this environmental impact indicator shall be used with care as the uncertainties on these results are high
as there is limited experience with the indicator. This EPD was created using a software tool.
References
Standards EN 13115: 2020 Windows - Classification of mechanical
properties - Racking, torsion and operating forces
EN 14351-1
EN 14351-1: 2016, Windows and doors - Product standard, EN 13049
performance characteristics - Part 1: windows and external EN 13049 2003 Windows - Soft and heavy body impact - Test
pedestrian doorsets method, safety requirements and classification
EN 12210
EN 12210: 2016 Windows and doors - Resistance to wind EN 15804
loads - classification EN 15804:2012+A2:2019+AC:2021, Sustainability of
construction works — Environmental Product Declarations —
EN ISO 10140 Core rules for the product category of construction products.
EN ISO 10140-1: 2021 Acoustics - Laboratory measurement of
sound insulation of building elements - Part 1: Application rules ISO 14025
for specific products EN ISO 14025:2011, Environmental labels and declarations —
Type III environmental declarations — Principles and
DIN EN ISO 10077 procedures.
DIN EN ISO 10077-2: 2017 Thermal performance of windows,
doors and shutters - Calculation of thermal transmittance - Part ECHA candidate list
2: Numerical method for frames ECHA candidate list [BSJ1] - Substances of Very High Concern
– SVHC (date 27.06.2024)
EN 12207 Candidate List of substances of very high concern for
EN 12207: 2016 Windows and doors - Air permeability - Authorisation (published in accordance with Article 59(10) of
Classification the REACH Regulation)
EN 13115 REGULATION (EU) No 528/2012
6 Environmental Product Declaration - Jansen AG - Janisol Primo window width x height: 1230 mm x 1480 mm
REGULATION (EU) No 528/2012 OF THE EUROPEAN LCA-Tool No.: IBU-JAN-202301-LT1-EN
PARLIAMENT AND OF THE COUNCIL Developed by Sphera Solutions GmbH
of 22 May 2012, concerning the making available on the market
and use of biocidal products IBU 2021
Institut
SBR 2011 Bauen und Umwelt e.V.: General Instructions for the EPD
SBR life cycle guide [SBR 2011] programme of Institut Bauen und Umwelt e.V., Version 2.0,
Berlin: Institut Bauen und Umwelt e.V., 2021
Further References www.ibu-epd.com
Sphera LCA FE Software (GaBi ts) PCR Part A
Sphera LCA software (GaBi ts) content update package (CUP) PCR - Part A: Calculation rules for the Life Cycle Assessment
version 2022.2 (https://www.gabi-software.com/support/gabi) and Requirements on the Background Report, version 1.3,
Institut Bauen und Umwelt e.V., 2021.
Sphera LCA Calculator Software (GaBi Envision)
GaBi Envision 5.0 Sphera Solution GmbH, the LCA, EPD and PCR Part B
Ecodesign tool, http://www.gabi- PCR – Part B: Requirements on the EPD for Windows and
software.com/international/software/gabi-envision/, 2022 doors, version 1.6, Institut Bauen und Umwelt e.V., www.bau-
umwelt.com, 2022
Jansen LCA tool
LCA tool for façades, windows & door
7 Environmental Product Declaration - Jansen AG - Janisol Primo window width x height: 1230 mm x 1480 mm
Publisher
Institut Bauen und Umwelt e.V. +49 (0)30 3087748- 0
Hegelplatz 1 info@ibu-epd.com
10117 Berlin www.ibu-epd.com
Germany
Programme holder
Institut Bauen und Umwelt e.V. +49 (0)30 3087748- 0
Hegelplatz 1 info@ibu-epd.com
10117 Berlin www.ibu-epd.com
Germany
Author of the Life Cycle Assessment
Sphera Solutions GmbH +49 711 341817-0
Hauptstraße 111- 113 info@sphera.com
70771 Leinfelden-Echterdingen www.sphera.com
Germany
Owner of the Declaration
JANSEN AG 0041717639113
Industriestrasse 34 sustainability@jansen.com
9463 Oberriet www.jansen.com
Switzerland
8 Environmental Product Declaration - Jansen AG - Janisol Primo window width x height: 1230 mm x 1480 mm
