ENVIRONMENTAL PRODUCT DECLARATION
as per ISO 14025 and EN 15804+A2
Owner of the Declaration JANSEN AG
Publisher Institut Bauen und Umwelt e.V. (IBU)
Programme holder Institut Bauen und Umwelt e.V. (IBU)
Declaration number EPD-JAN-20240295-CBA1-EN
Issue date 29.11.2024
Valid to 28.11.2029
Janisol C4 door width x height: 1230 mm x 2180 mm
Jansen AG
www.ibu-epd.com | https://epd-online.com
General Information
Jansen AG Janisol C4 door width x height: 1230 mm x 2180
mm
Programme holder Owner of the declaration
IBU – Institut Bauen und Umwelt e.V. JANSEN AG
Hegelplatz 1 Industriestrasse 34
10117 Berlin 9463 Oberriet
Germany Switzerland
Declaration number Declared product / declared unit
EPD-JAN-20240295-CBA1-EN 1 m2 Jansen Janisol C4 with a grammage of 114.06 kg/m². The actual
reference size of the declared single leaf door has dimensions of width x
height: 1230 mm x 2180 mm.
This declaration is based on the product category rules: Scope:
Windows and doors , 01.08.2021 The environmental product declaration refers to a single leaf door type
(PCR checked and approved by the SVR) Jansen Janisol C4 in specific dimension width x height. The characteristic
values used for the system components Janisol C4 in the LCA are
provided by Jansen AG.
Issue date
The declared product is defined according to the profile series and product
29.11.2024
characteristics.
The location of the production site is Oberriet/ Switzerland.
Valid to
This EPD was created with the help of a semi-automatic LCA-Tool.
28.11.2029 The owner of the declaration shall be liable for the underlying information
and evidence; the IBU shall not be liable with respect to manufacturer
information, life cycle assessment data and evidences.
The EPD was created according to the specifications of EN 15804+A2. In
the following, the standard will be simplified as EN 15804.
Verification
The standard EN 15804 serves as the core PCR
Independent verification of the declaration and data according to ISO
14025:2011
Dipl.-Ing. Hans Peters internally X externally
(Chairman of Institut Bauen und Umwelt e.V.)
Florian Pronold Matthias Schulz,
(Managing Director Institut Bauen und Umwelt e.V.) (Independent verifier)
1 Environmental Product Declaration - Jansen AG - Janisol C4 door width x height: 1230 mm x 2180 mm
Product
According to the CE marking, the following structural data for
Product description/Product definition
the element must be stated:
Janisol C4 is a complete profile system for glazed single- and
Constructional data
double-leaf fire resistant doors and glazing. The profiles with a
basic depth of just 70 mm achieve security classifications up to Name Value Unit
EI90 due to the innovative fire-resistant infill panels. The Resistance to wind load acc. to EN
4 class
profiles are filled with a ceramic fire board in the factory. The 12210
appearance of the Janisol C4 fire-resistant construction is Water tightness acc. to EN 12208 4A class
identical to the other Jansen fire protection barriers and the
Sound insulation class according to EN Rw 43 db
thermally insulated Janisol systems. This declaration describes -
ISO 10140 (-1;-4)
the following element in Janisol C4:
Heat transfer coefficient acc. to DIN EN
Product: Jansen Janisol C4, single leaf door 2.9 W/(m2K)
ISO 10077-2
Face width: 107.5 mm
Construction depth: 70 mm Air permeability acc. to EN 12207 4 class
Width x height: 1230 mm x 2180 mm Classification of strength requirements
4 class
CE marking according to EN 14351-1 acc. to EN 1192
Mechanical durability acc. to EN 12400 6 class
For the placing on the market in the the European Union/
Operating forces acc. to EN 12217 2 class
European Free Trade Association EU/EFTA the CPR (EU) No.
Fire resistance class acc. to DIN EN
305/2011/ applies. The products require a declaration of EI60/EI90 class
1634-1 / EN13501-2
performance taking into account the harmonized product
standard EN 14351-1 windows and doors and a CE marking. Product according to the CPR, based on an EN: Performance
The respective national regulations apply to the use. With this data of the product in accordance with the declaration of
declaration the following element is declared: performance with respect to its essential characteristics
according to EN 14351-1, doors. Other constructional data are
not relevant for this product.
Base materials/Ancillary materials
JANSEN Janisol C4 door is made of the following materials:
• Glazing approx. 65%
• Steel approx. 17%
• Stainless steel approx. <1%
• Plastics and fillers approx. 3%
• Multi-Materials approx. 14%
The percentages relate to the most frequently sold product with
an opening of 2.68 m2. The percentages stated may vary
depending on the product type and dimensions.
Does the product or at least one part product contain materials
from the ECHA candidate list of materials which are especially
problematic for approval: Substances of Very High Concern –
SVHC (date 27.06.2024) above a mass % of 0.1: no.
This product/article/at least one partial article contains other
carcinogenic, mutagenic, reprotoxic (CMR) substances in
categories 1A or 1B which are not on the candidate list,
exceeding 0.1 percentage by mass: no.
Biocide products were added to this construction product or it
has been treated with biocide products (this then concerns a
treated product as defined by the (EU) Ordinance on Biocide
Products No. 528/2012): no.
Reference service life
Application
According to SBR 2011 regarding the specific material
The Jansen Janisol C4 door can be integrated for building
characteristics of steel windows and doors, the reference
ventilation and light transmission and it meets all the
service life is 75 years (SBR 2011). The practical service life
requirements of an interior or exterior wall without taking over
may well be longer. Conditions for a long service life are regular
load-bearing functions.
maintenance, care and upkeep of the product. The specified
service life is independent of the manufacturer's warranty.
Technical Data
LCA: Calculation rules
2 Environmental Product Declaration - Jansen AG - Janisol C4 door width x height: 1230 mm x 2180 mm
environmental burdens).
Declared Unit
The declared unit is a 1 m2 of Janisol C4 door element. Module C2 - considers 50 km truck transport to waste
The actual reference size of the declared door element has processing. The transport distance can
dimensions of 1230 mm x 2180 mm. be modified project-specific if required by linear scaling.
Declared unit
Modules C3 and C4 - consider waste processing and/or
Name Value Unit
disposal with the following scenarios:
Declared unit 1 m2
• Scenario 0: 100% thermal treatment of all raw materials
Grammage 114.06 kg/m2 with heating value including plastic system parts and
Layer thickness 0.07 m 100% recycling of metal system components (C3).
Landfill of all materials without heating value (except
Other declared units are allowed if the conversion is shown
metals) including glazing (C4). For mineral based
transparently.
components (i.e. gypsum board), construction waste
processing (shredding) and material recycling as filling
For inhomogeneous components made of different materials,
material (incl. benefits for substitution of gravel in
the conversion to other dimensions with factors leads to
Module (D) is considered, assuming 3% recycling
deviations compared to the exact calculation. The frame
losses are sent to landfill (C4).
percentage is 30.02% and the ground reference is 0.086m².
Frame percentage = Frame surface / total area * 100 [%] • Scenario 1 (module C3/1): 100% recycling of plastic
Ground reference = Element depth x element width [m²] system parts (excluding e-waste sent to incineration)
and 100% recycling of metal system components.
System boundary Landfill of all materials without heating value (except
Type of EPD according to EN 15804: "cradle to gate with metals) including glazing (C4/1). For mineral based
options, modules C1–C4, and module D". The following components (i.e. gypsum board), construction waste
modules are declared: A1–A3, C, D and additional modules: processing (shredding) and material recycling as filling
A4, A5 and B6. material (incl. benefits for substitution of gravel in
Module D/1) are considered, assuming 3% recycling
Production (modules A1-A3): losses are sent to landfill (C4/1).
This module considers the provision of all relevant door Modules C4 & C4/1 are identical.
components (i.e. metal profiles/components, plastic
parts/profiles and glazing) and raw materials including their Benefits and loads beyond the product system boundary
transport to the declared production plant. This considers the (module D):
manufacturing and assembly of these components, including
waste processing up to the end-of-waste state. The impact of Considers credits and loads from the recycling of the metal
packaging materials is also covered by this module. components and mineral based components (i.e. gypsum
board) as filling material (incl. benefits for the substitution of
Transport to the construction site (module A4): gravel (duplicated in D and D/1) and the recycling of the plastic
system parts/profiles (D/1). Avoided burdens from the thermal
A distance of 100 km is considered for the transport of the treatment of all raw materials with heating value (including
packed finished product via truck. The transport distance can plastic system parts/profiles) (D) and packaging treatment
be modified project-specific if required by linear scaling. (duplicated in D and D/1) under European conditions are
considered. This affects only the rate of primary materials (no
Installation (module A5): secondary materials).
Treatment and disposal of packaging material is considered in Geographic Representativeness
this module. Credits for potential avoided burdens due to Land or region, in which the declared product system is
energy substitution of electricity and thermal energy generation manufactured, used or handled at the end of the product´s
are declared in module D under European conditions and lifespan: Europe
affects only the rate of primary materials (no secondary
materials).
Comparability
Operational energy use (module B6): Basically, a comparison or an evaluation of EPD data is only
Electric consumption for operating the motorised door is possible if all the data sets to be compared were created
considered. Its impacts are calculated per year. according to EN 15804 and the building context, respectively
the product-specific characteristics of performance, are taken
EoL stage (modules C1-C4): into account. The following background database has been
used for the LCA calculation: Sphera LCA software (GaBi ts)
Module C1 - considers manual deconstruction (without content update package (CUP) version 2022.2
LCA: Scenarios and additional technical information
Name Value Unit
Characteristic product properties of biogenic carbon
kg
No biogenic carbon is reported in the product. The biogenic Biogenic carbon content in product -
C
carbon content in the accompanying packaging for 1 m2 Janisol
Biogenic carbon content in accompanying kg
C4 door is declared below. 0.01083
packaging C
Information on describing the biogenic Carbon Content at
Note: 1 kg of biogenic carbon is equivalent to 44/12 kg of CO .
factory gate 2
3 Environmental Product Declaration - Jansen AG - Janisol C4 door width x height: 1230 mm x 2180 mm
board), construction waste processing (shredding) and material
The following technical information is a basis for the declared recycling as filling material (incl. benefits for substitution of
modules. The values refer to the declared unit of 1 m2 of gravel in Module D) are considered, assuming 3% recycling
Jansen Janisol C4 door. losses are sent to landfill (C4).
Scenario 1 considers 100% recycling of plastic system parts
Transport to the building site (A4)
(excluding e-waste sent to incineration) and 100% recycling of
Name Value Unit metal system components (C3/1). Landfill of all materials
Litres of fuel 0.212 l/100km without heating value (except metals) including glazing (C4/1).
Transport distance 100 km For mineral based components (i.e. gypsum board),
construction waste processing (shredding) and material
Capacity utilisation (including empty runs) 61 %
recycling as filling material (incl. benefits for substitution of
Gross weight of packed products transported 114.09 kg
gravel in Module D/1) are considered, assuming 3% recycling
losses are sent to landfill (C4/1). Modules C4 and C4/1 are
Installation into the building (A5)
identical. The recycling of plastics scenario declared in this
Treatment and disposal of packaging material is considered in
EPD is currently considered a scenario that is not widely
this module.
available in reality due to economic viability limitations
The values refer to the declared unit of 1 m2 of Janisol C4 door.
associated with higher costs of sorting smaller shares of
Name Value Unit plastics such as those present in the declared product.
Polyethylene (waste packaging to incineration) 0.00233 kg Name Value Unit
Cardboard box (waste packaging to incineration) 0.01117 kg EoL scenario 0 (modules C3 and C4)
Wood (waste packaging to incineration) 0.01473 kg Recycling (C3) 35.94 kg
According to SBR 2011 regarding the specific material Energy recovery (C3) 3.21 kg
characteristics of steel windows and doors, the reference Landfilling (C4) 75.02 kg
service life is 75 years (SBR 2011). The practical service life
EoL scenario 1 (modules C3/1 and C4/1)
may well be longer. Conditions for a long service life are regular
Recycling (C3/1) 38.98 kg
maintenance, care and upkeep of the product. The specified
service life is independent of the manufacturer's warranty. Energy recovery (C3/1) 0.17 kg
Landfilling (C4/1) 75.02 kg
Reference service life
Name Value Unit Reuse, recovery and/or recycling potentials (D), relevant
scenario information
Life Span (according to SBR 2011) 75 a
Operational energy use (B6) Module D includes the credits and loads from the recycling of
the metal components and mineral based components (i.e.
The value below refers to the declared unit of 1 m2 of Jansen
gypsum board) as filling material (incl. benefits for substitution
Janisol C4 door.
of gravel (duplicated in D and D/1) and the recycling of the
Name Value Unit
plastic system parts/profiles (D/1). Avoided burdens from the
Electricity consumption (per year) 72.39 MJ thermal treatment of all raw materials with heating value
(including plastic system parts/profiles) (D) and packaging
End of life (C1-C4)
treatment (duplicated in D and D/1) under European conditions
For the End-of-Life stage two scenarios are considered. are considered. This affects only the rate of primary materials
Scenario 0 considers 100% thermal treatment of all raw (no secondary materials). A waste incineration plant with R1-
materials with heating value including plastic system parts and value > 0.6 is assumed.
100% recycling of metal system components (C3). Landfill of all For recycling, a collection rate of 100% is considered.
materials without heating value (except metals) including
glazing (C4). For mineral based components (i.e. gypsum
4 Environmental Product Declaration - Jansen AG - Janisol C4 door width x height: 1230 mm x 2180 mm
LCA: Results
Results provided in this section are presented in relation to 1 m2 of door type Jansen Janisol C4 (reference dimensions 1230 mm x
2180 mm).
For the operational energy use (B6), electric consumption for operating the motorised door is considered. Its impacts are calculated per
year.
For the End-of-Life stage, two scenarios are considered:
C3 - considers 100% recycling of metal system components (duplicated in D and D/1) and 100% thermal treatment of all raw materials
with heating value including plastic system parts. For mineral based components (i.e. gypsum board), construction waste processing
(shredding) and material recycling as filling material is considered.
C3/1 - considers 100% recycling of metal system components (duplicated in D and D/1) and 100% recycling of plastic system parts
(excluding e-waste sent to incineration). For mineral based components (i.e. gypsum board), construction waste processing
(shredding) and material recycling as filling material is considered.
C4 and C4/1 - consider landfill of all materials without heating value (except metals) including glazing and recycling losses from mineral
based components (i.e. gypsum board). Modules C4 and C4/1 are identical.
D - considers credits and loads from the recycling of the metal components and mineral based components (i.e. gypsum board) as
filling material (incl. benefits for the substitution of gravel (duplicated in D and D/1)). Avoided burdens from packaging treatment
(duplicated in D and D/1) and thermal treatment of all raw materials with heating value (including plastic system parts/profiles) are
considered.
D/1 - considers credits and loads from the recycling of the metal components and mineral based components (i.e. gypsum board) as
filling material (incl. benefits for the substitution of gravel (duplicated in D and D/1)) and the recycling of the plastic system
parts/profiles. Avoided burdens from packaging treatment (duplicated in D and D/1) are considered.
DESCRIPTION OF THE SYSTEM BOUNDARY (X = INCLUDED IN LCA; MND = MODULE OR INDICATOR NOT DECLARED; MNR
= MODULE NOT RELEVANT)
Benefits and
Construction loads beyond
Product stage Use stage End of life stage
process stage the system
boundaries
la ire ta m w a Ry lp p u s tro p s n a rT g n iru tc a fu n a M e h t m o rf tro p s n a rTe tis e h t o t e ta g y lb m e s s A e s U e c n a n e tn ia M ria p e R tn e m e c a lp e R tn e m h s ib ru fe R y g re n e la n o ita re p Oe s u re ta w la n o ita re p Oe s u n o itc u rts n o c -e Dn o itilo m e d tro p s n a rT g n is s e c o rp e ts a W la s o p s iD -e s u e R-y re v o c e R-g n ilc y c e Rla itn e to p
A1 A2 A3 A4 A5 B1 B2 B3 B4 B5 B6 B7 C1 C2 C3 C4 D
X X X X X MND MND MNR MNR MNR X MND X X X X X
RESULTS OF THE LCA - ENVIRONMENTAL IMPACT according to EN 15804+A2: 1 m2 Janisol C4 door (114.06 kg/m2)
Parameter Unit A1-A3 A4 A5 B6 C1 C2 C3 C3/1 C4 C4/1 D D/1
GWP-total kg CO 2 eq 1.96E+02 6.89E-01 4.74E-02 2.17E+01 0 3.44E-01 8.57E+00 1.65E-01 1.13E+00 1.13E+00 -2.19E+01 -2.01E+01
GWP-fossil kg CO 2 eq 1.95E+02 6.82E-01 8.07E-03 2.17E+01 0 3.41E-01 8.57E+00 1.65E-01 1.12E+00 1.12E+00 -2.19E+01 -2.01E+01
GWP-
biogenic kg CO 2 eq 7.65E-01 2.88E-03 3.93E-02 1.28E-02 0 1.44E-03 4.54E-04 3.59E-05 3.77E-03 3.77E-03 -1.05E-02 -8.26E-04
GWP-luluc kg CO 2 eq 4.8E-02 3.81E-03 1.29E-07 1.41E-03 0 1.9E-03 2.04E-04 1.81E-04 2.07E-03 2.07E-03 -2.63E-03 -2.83E-03
kg CFC11
ODP 4.06E-10 4.09E-14 4.07E-15 2.14E-10 0 2.05E-14 7.46E-13 1.04E-13 2.63E-12 2.63E-12 -2.55E-11 -2.97E-12
eq
AP mol H+ eq 9.47E-01 6.5E-04 8.87E-06 3.18E-02 0 3.25E-04 1.56E-03 2.36E-04 7.94E-03 7.94E-03 -5.44E-02 -5.44E-02
EP-
kg P eq 2.71E-04 2.04E-06 1.1E-09 9.73E-06 0 1.02E-06 3.2E-07 1.42E-07 1.9E-06 1.9E-06 -9.3E-06 -8.16E-06
freshwater
EP-marine kg N eq 2.57E-01 2.02E-04 2.97E-06 8.7E-03 0 1.01E-04 4.65E-04 1.06E-04 2.03E-03 2.03E-03 -8.71E-03 -8.72E-03
EP-terrestrial mol N eq 2.98E+00 2.43E-03 4.12E-05 9.3E-02 0 1.22E-03 7.45E-03 1.19E-03 2.23E-02 2.23E-02 -8.09E-02 -8.1E-02
kg NMVOC
POCP 6.38E-01 5.66E-04 8E-06 2.46E-02 0 2.83E-04 1.26E-03 2.87E-04 6.17E-03 6.17E-03 -3.29E-02 -3.61E-02
eq
ADPE kg Sb eq 8.02E-03 5.71E-08 9.95E-11 2.58E-06 0 2.85E-08 5.9E-08 4.34E-08 1.15E-07 1.15E-07 -4.25E-04 -4.25E-04
ADPF MJ 2.69E+03 9.13E+00 1.12E-02 4.6E+02 0 4.56E+00 2.21E+00 8.36E-01 1.47E+01 1.47E+01 -2.33E+02 -2.73E+02
m3 world eq
WDP 1.63E+01 6.13E-03 5.4E-03 1.62E+00 0 3.06E-03 8.13E-01 3.36E-02 1.23E-01 1.23E-01 -3.93E+00 -4.14E+00
deprived
GWP = Global warming potential; ODP = Depletion potential of the stratospheric ozone layer; AP = Acidification potential of land and water; EP =
Eutrophication potential; POCP = Formation potential of tropospheric ozone photochemical oxidants; ADPE = Abiotic depletion potential for non-fossil
resources; ADPF = Abiotic depletion potential for fossil resources; WDP = Water (user) deprivation potential)
RESULTS OF THE LCA - INDICATORS TO DESCRIBE RESOURCE USE according to EN 15804+A2: 1 m2 Janisol C4 door
(114.06 kg/m2)
Parameter Unit A1-A3 A4 A5 B6 C1 C2 C3 C3/1 C4 C4/1 D D/1
PERE MJ 2.63E+02 5.19E-01 3.92E-01 6.64E+01 0 2.59E-01 4.34E-01 8.79E-02 2.2E+00 2.2E+00 -1.51E+01 4.37E-01
PERM MJ 3.9E-01 0 -3.9E-01 0 0 0 0 0 0 0 0 0
PERT MJ 2.64E+02 5.19E-01 2.57E-03 6.64E+01 0 2.59E-01 4.34E-01 8.79E-02 2.2E+00 2.2E+00 -1.51E+01 4.37E-01
PENRE MJ 2.58E+03 9.15E+00 1.18E-01 4.6E+02 0 4.57E+00 1.13E+02 1.11E+02 1.47E+01 1.47E+01 -2.33E+02 -2.73E+02
5 Environmental Product Declaration - Jansen AG - Janisol C4 door width x height: 1230 mm x 2180 mm
PENRM MJ 1.11E+02 0 -1.07E-01 0 0 0 -1.1E+02 -1.1E+02 0 0 0 0
PENRT MJ 2.69E+03 9.15E+00 1.12E-02 4.6E+02 0 4.57E+00 2.21E+00 8.37E-01 1.47E+01 1.47E+01 -2.33E+02 -2.73E+02
SM kg 1.18E+01 0 0 0 0 0 0 0 0 0 9.95E+00 1.15E+01
RSF MJ 0 0 0 0 0 0 0 0 0 0 0 0
NRSF MJ 0 0 0 0 0 0 0 0 0 0 0 0
FW m3 5.57E-01 5.87E-04 1.27E-04 1.01E-01 0 2.93E-04 1.91E-02 8.05E-04 3.73E-03 3.73E-03 -1.08E-01 -1.07E-01
PERE = Use of renewable primary energy excluding renewable primary energy resources used as raw materials; PERM = Use of renewable primary
energy resources used as raw materials; PERT = Total use of renewable primary energy resources; PENRE = Use of non-renewable primary energy
excluding non-renewable primary energy resources used as raw materials; PENRM = Use of non-renewable primary energy resources used as raw
materials; PENRT = Total use of non-renewable primary energy resources; SM = Use of secondary material; RSF = Use of renewable secondary fuels;
NRSF = Use of non-renewable secondary fuels; FW = Use of net fresh water
RESULTS OF THE LCA – WASTE CATEGORIES AND OUTPUT FLOWS according to EN 15804+A2:
1 m2 Janisol C4 door (114.06 kg/m2)
Parameter Unit A1-A3 A4 A5 B6 C1 C2 C3 C3/1 C4 C4/1 D D/1
HWD kg 2.77E-07 4.38E-11 1.09E-12 3.29E-08 0 2.19E-11 1.52E-10 1.57E-11 7.54E-10 7.54E-10 -8.54E-09 -5.78E-09
NHWD kg 1.83E+01 1.31E-03 7.16E-04 9.77E-02 0 6.56E-04 1.33E-01 2.08E-02 7.51E+01 7.51E+01 1.18E+00 1.27E+00
RWD kg 5.9E-02 1.13E-05 6.38E-07 7.64E-02 0 5.63E-06 7.8E-05 1.58E-05 1.63E-04 1.63E-04 -5.59E-03 -1.07E-03
CRU kg 0 0 0 0 0 0 0 0 0 0 0 0
MFR kg 5.87E-01 0 0 0 0 0 3.59E+01 3.9E+01 0 0 0 0
MER kg 0 0 0 0 0 0 0 0 0 0 0 0
EEE MJ 0 0 5.41E-02 0 0 0 1.57E+01 1.61E-01 0 0 0 0
EET MJ 0 0 9.69E-02 0 0 0 3.03E+01 3.27E-01 0 0 0 0
HWD = Hazardous waste disposed; NHWD = Non-hazardous waste disposed; RWD = Radioactive waste disposed; CRU = Components for re-use;
MFR = Materials for recycling; MER = Materials for energy recovery; EEE = Exported electrical energy; EET = Exported thermal energy
RESULTS OF THE LCA – additional impact categories according to EN 15804+A2-optional:
1 m2 Janisol C4 door (114.06 kg/m2)
Parameter Unit A1-A3 A4 A5 B6 C1 C2 C3 C3/1 C4 C4/1 D D/1
Disease
PM 6.8E-06 3.93E-09 4.66E-11 2.84E-07 0 1.97E-09 1.24E-08 4.54E-09 9.77E-08 9.77E-08 -6.71E-07 -6.73E-07
incidence
kBq U235
IR 9.37E+00 1.65E-03 1.04E-04 1.12E+01 0 8.26E-04 1.13E-02 2.35E-03 1.82E-02 1.82E-02 -6.11E-01 1.58E-01
eq
ETP-fw CTUe 4.07E+03 6.34E+00 5.14E-03 1.41E+02 0 3.17E+00 1.16E+00 5.66E-01 8.22E+00 8.22E+00 -3.18E+01 -7.01E+01
HTP-c CTUh 9.2E-08 1.28E-10 3.37E-13 2.59E-09 0 6.38E-11 7.58E-11 1.37E-11 1.25E-09 1.25E-09 -8.24E-09 -9.06E-09
HTP-nc CTUh 2.29E-06 6.61E-09 1.27E-11 1.32E-07 0 3.3E-09 3.59E-09 7.24E-10 1.39E-07 1.39E-07 -2.99E-07 -3.58E-07
SQP SQP 2.18E+02 3.14E+00 3.24E-03 4.22E+01 0 1.57E+00 6E-01 1.99E-01 3.05E+00 3.05E+00 -1.5E+01 -5.56E+00
PM = Potential incidence of disease due to PM emissions; IR = Potential Human exposure efficiency relative to U235; ETP-fw = Potential comparative
Toxic Unit for ecosystems; HTP-c = Potential comparative Toxic Unit for humans (cancerogenic); HTP-nc = Potential comparative Toxic Unit for humans
(not cancerogenic); SQP = Potential soil quality index
Disclaimer 1 – for the indicator 'Potential Human exposure efficiency relative to U235'.This impact category deals mainly with the
eventual impact of low dose ionizing radiation on human health of the nuclear fuel cycle. It does not consider effects due to possible
nuclear accidents, occupational exposure or radioactive waste disposal in underground facilities. Potential ionizing radiation from the
soil, from radon and from some construction materials is also not measured by this indicator.
Disclaimer 2 – for the indicators 'abiotic depletion potential for non-fossil resources', 'abiotic depletion potential for fossil resources',
'water (user) deprivation potential, deprivation-weighted water consumption', 'potential comparative toxic unit for ecosystems', 'potential
comparative toxic unit for humans – cancerogenic', 'Potential comparative toxic unit for humans - not cancerogenic', 'potential soil
quality index'. The results of this environmental impact indicator shall be used with care as the uncertainties on these results are high
as there is limited experience with the indicator. This EPD was created using a software tool.
References
Standards EN ISO 14025:2011, Environmental labels and declarations —
Type III environmental declarations — Principles and
EN 14351-1 procedures.
EN 14351-1:2016, Windows and doors - Product standard,
performance characteristics - Part 1: windows and external EN 12210
pedestrian doorsets EN 12210: 2016 Windows and doors - Resistance to wind
loads - classification
EN 16034
EN 16034:2014, pedestrian doorsets, industrial, commercial, EN 12208
garage doors and openable windows - Product standard, DIN EN 12208 Windows and doors - Watertightness -
performance characteristics - Fire resistance and/or smoke Classification
control characteristics
EN ISO 10140
EN 15804 EN ISO 10140-1: 2021 Acoustics - Laboratory measurement of
EN 15804:2012+A2:2019+AC:2021, Sustainability of sound insulation of building elements - Part 1: Application
construction works — Environmental Product Declarations — rulesfor specific products
Core rules for the product category of construction products.
DIN EN ISO 10077-2
ISO 14025 DIN EN ISO 10077-2: 2017 Thermal performance of windows,
6 Environmental Product Declaration - Jansen AG - Janisol C4 door width x height: 1230 mm x 2180 mm
doors and shutters - Calculation of thermal transmittance - REACH Regulation)REGULATION (EU) No
Part2: Numerical method for frames 528/2012REGULATION (EU) No 528/2012 OF THE
EUROPEANPARLIAMENT AND OF THE COUNCIL, of 22 May
EN 12207 2012, concerning the making available on the market and use
EN 12207: 2016 Windows and doors - Air permeability - of biocidal products
Classification
SBR 2011
EN 1192 SBR life cycle guide [SBR 2011]
EN 1192: 2000 Doors - Classification of strength requirements
Further References
EN 1191
EN 1191: 2012 Windows and doors - Resistance to repeated Sphera LCA FE Software (GaBi ts)
opening and closing - Test method GaBi ts dataset documentation for the software-system and
databases, LBP, University of Stuttgart and thinkstep,
EN 1603 Leinfelden-Echterdingen, 2023 (https://www.gabi-
DIN EN 1603:2013-05 Thermal insulating products for building software.com/support/gabi)
applications - Determination of dimensional stability under
constant normal laboratory conditions Sphera LCA Calculator Software (GaBi Envision)
GaBi Envision 5.0 Sphera Solution GmbH, the LCA, EPD and
EN 13115 Ecodesign tool, http://www.gabi-
EN 13115: 2020 Windows - Classification of mechanical software.com/international/software/gabi-envision/, 2022
properties - Racking, torsion and operating forces.
DIN EN 1634-1
DIN EN 1634-1 Fire resistance and smoke control tests for door Jansen LCA tool
and shutter assemblies, openable windows and elements of LCA tool for façades, windows & door
building hardware - Part 1: Fire resistance test for door and LCA-Tool No.: IBU-JAN-202301-LT1-EN
shutter assemblies and openable windows Developed by Sphera Solutions GmbH
IBU 2021
EN 13501-2 Institut Bauen und Umwelt e.V.: General Instructions for the
EN 13501-2: 2021 Fire classification of construction products EPD programme of Institut Bauen und Umwelt e.V., Version
and building elements - Part 2: Classification using data from 2.0, Berlin: Institut Bauen und Umwelt e.V., 2021
fire resistance and/or smoke control tests, excluding ventilation
services www.ibu-epd.com
EN 1627 PCR Part A
DIN EN 1627:2011-09 Pedestrian doorsets, windows, curtain PCR - Part A: Calculation rules for the Life Cycle Assessment
walling, grilles and shutters - Burglar resistance - Requirements and Requirements on the Background Report, version 1.3,
and classification Institut Bauen und Umwelt e.V., 08-2021.
ECHA candidate list
ECHA candidate list [BSJ1] - Substances of Very High PCR Part B
Concern– SVHC (date 27.06.2024) PCR – Part B: Requirements on the EPD for Windows and
Candidate List of substances of very high concern for doors, version 1.6, Institut Bauen und Umwelt e.V., 2022
Authorisation (published in accordance with Article 59(10) ofthe
7 Environmental Product Declaration - Jansen AG - Janisol C4 door width x height: 1230 mm x 2180 mm
Publisher
Institut Bauen und Umwelt e.V. +49 (0)30 3087748- 0
Hegelplatz 1 info@ibu-epd.com
10117 Berlin www.ibu-epd.com
Germany
Programme holder
Institut Bauen und Umwelt e.V. +49 (0)30 3087748- 0
Hegelplatz 1 info@ibu-epd.com
10117 Berlin www.ibu-epd.com
Germany
Author of the Life Cycle Assessment
Sphera Solutions GmbH +49 (0)711 341817-0
Hauptstraße 111- 113 info@sphera.com
70771 Leinfelden-Echterdingen www.sphera.com
Germany
Owner of the Declaration
JANSEN AG 0041717639113
Industriestrasse 34 sustainability@jansen.com
9463 Oberriet www.jansen.com
Switzerland
8 Environmental Product Declaration - Jansen AG - Janisol C4 door width x height: 1230 mm x 2180 mm
