Environmental product declaration
in accordance with ISO 14025 and EN 15804+A2
Jura 15-48 IP69K DALI
Owner of the declaration: Program operator:
Betek Norge AS The Norwegian EPD Foundation
Product: Declaration number:
Jura 15-48 IP69K DALI
NEPD-9294-8879
Declared unit:
1 pcs Registration number:
This declaration is based on Product Category Rules: NEPD-9294-8879
CEN Standard EN 15804:2012+A2:2019 serves as core
Issue date: 04.03.2025
PCR
The Norwegian EPD Foundation IBU PCR - Part B for luminaires, lamps, and components Valid to: 04.03.2030
for luminaires
EPD software:
LCAno EPD generator ID: 759172
1 / 13
General information
Product Owner of the declaration:
Jura 15-48 IP69K DALI Betek Norge AS
Contact person: Olav Klepp
Phone: +47 41560701
e-mail: ok@betek-norge.no
Manufacturer:
Betek Norge AS
Juraveien 4
4636 Kristiansand, Norway
Program operator:
The Norwegian EPD Foundation
Post Box 5250 Majorstuen, 0303 Oslo, Norway Place of production:
Phone: +47 977 22 020 Betek production site, (China)
web: www.epd-norge.no
Shenzhen, China
Declaration number:
Management system:
NEPD-9294-8879
This declaration is based on Product Category Rules:
CEN Standard EN 15804:2012+A2:2019 serves as core PCR Organisation no:
IBU PCR - Part B for luminaires, lamps, and components for 980832481
luminaires
Statement of liability:
​
The owner of the declaration shall be liable for the underlying
information and evidence. EPD Norway shall not be liable with respect Issue date:
to manufacturer information, life cycle assessment data and
evidences. 04.03.2025
Valid to:
Declared unit:
04.03.2030
1 pcs Jura 15-48 IP69K DALI
Year of study:
Declared unit with option:
2023
A1,A2,A3,A4,A5,B6,C1,C2,C3,C4,D
Comparability:
EPD of construction products may not be comparable if they not
comply with EN 15804 and seen in a building context.
Functional unit:
Jura 15-48 IP69K DALI luminaire manufactured and installed, used Development and verification of EPD:
according to a specific lighting regime over 15 years, including waste The declaration is created using EPD tool lca.tools ver EPD2021.09,
treatment at end-of-life. developed by LCA.no. The EPD tool is integrated in the company's
management system, and has been approved by EPD Norway.
General information on verification of EPD from EPD tools:
Independent verification of data, other environmental information Developer of EPD: Olav Klepp
and the declaration according to ISO 14025:2010, § 8.1.3 and § 8.1.4.
Verification of each EPD is made according to EPD-Norway’s Reviewer of company-specific input data and EPD:​ Torgeir Aasen
guidelines for verification and approval requiring that tools are i)
integrated into the company's environmental management system, ii)
the procedures for use of the EPD tool are approved by EPD-Norway,
and iii) the process is reviewed annually by an independent third Approved:
party verifier. See Appendix G of EPD-Norway's General Programme
Instructions for further information on EPD tools
Verification of EPD tool:
Independent third party verification of the EPD tool, background data Håkon Hauan, CEO EPD-Norge
and test-EPD in accordance with EPDNorway's procedures and
guidelines for verification and approval of EPD tools. Approval
number: NEPDT41.
Third party verifier:
Vito D’Incognito, Take Care International
2 / 13
(no signature required)
Product
Product description:
Certified with an IP69K rating, Jura is built to withstand high pressure, extreme temperature fluctuations, and powerful water jets. This makes it a
reliable choice for demanding environments such as car washes, agricultural facilities, and swimming pools. Jura is a dependable tubular luminaire
that combines functionality with simplicity. Its unique round design and clamp-based mounting system allow for an effortless installation process
without the need for additional angle brackets.
Product specification
Equipped with an integrated DALI driver, Jura offers advanced lighting control and dimming capabilities directly through your existing DALI
system. For enhanced installation efficiency, the luminaire features through-wiring with 5×1.5mm² connections and entry points on both sides,
ensuring a smooth and streamlined setup process. Key features: Durability: IP69K-certified for high-pressure cleaning, extreme environments, and
wet conditions. Ease of installation: Simple clamp system eliminates the need for extra brackets. Advanced control: Integrated DALI driver for
precise lighting control and dimming. Streamlined wiring: Through-wired with 5×1.5mm² and dual-side entry points for fast and efficient
installation.
Materials kg %
Copper conductor 0,00040 0,018
Electronic - Cable 0,17 8,27
Electronic - LED chip 0,0057 0,27
Electronic - LED driver 0,17 8,33
Electronic - LED plate 0,096 4,51
Electronic component 0,11 5,44
Plastic - Plexiglass (PMMA) 0,75 35,69
Plastic - Polyamide 0,0010 0,048
Rubber, synthetic 0,0017 0,079
Metal - Aluminium 0,62 29,30
Metal - Stainless steel 0,15 7,12
Silicone 0,013 0,64
Plastic - Polycarbonate (PC) 0,0052 0,24
Total 2,12 100,00
Packaging kg %
Packaging - Cardboard 0,41 88,28
Packaging - Paper 0,06 11,72
Total incl. packaging 2,60 100,00
Technical data:
Lumen: 7680 Lm
Power: 48 W
Lumen/watt: 160 Lm/W
Color temperature: 4000 K
Lifespan: 100,000h L80B10
Color rendering: 80
Driver: DALI
LxWxH: 1589x70x70 mm
Protection class: IP69K
MacAdamstep: 3
Light spread: 120°
Driver included: Yes
Sensor: -
UGR: -
Optics: Opal
Hole-making: -
Isosafe: -
Through-wiring: 5x1.5mm²
Mounting method: Ceiling and Wall
Insulation class: I
Market:
Norway
Reference service life, product
15 years (100 000 hours)
Reference service life, building or construction works
N.A
3 / 13
LCA: Calculation rules
Declared unit:
1 pcs Jura 15-48 IP69K DALI
Cut-off criteria:
All major raw materials and all the essential energy is included. The production processes for raw materials and energy flows with very small
amounts (less than 1%) can be excluded. These cut-off criteria do not apply for hazardous materials and substances.
Allocation:
The allocation is made in accordance with the provisions of EN 15804. Incoming energy and water and waste production in-house is allocated
equally among all products through mass allocation. Effects of primary production of recycled materials is allocated to the main product in which
the material was used. The recycling process and transportation of the material is allocated to this analysis.
Data quality:
Specific data for the product composition are provided by the manufacturer. The data represent the production of the declared product and were
collected for EPD development in the year of study. Background data is based on EPDs according to EN 15804 and different LCA databases. The
data quality of the raw materials in A1 is presented in the table below.
Materials Source Data quality Year
Copper conductor ecoinvent 3.6 Database 2019
Database +
Electronic - Cable Ecoinvent 3.6 Supplier 2019
Information
Scientific
Electronic - LED chip Scholand et al. (2012) + Ecoinvent 3.6 literature + 2017
database
Supplier data +
Electronic - LED driver Product composition + ecoinvent 3.6 2019
database
Electronic - LED plate ecoinvent 3.6 Database 2019
Electronic component ecoinvent 3.6 Database 2019
Metal - Aluminium ecoinvent 3.6 Database 2019
Metal - Stainless steel Modified ecoinvent 3.6 Database 2019
Packaging - Cardboard Modified ecoinvent 3.6 Database 2019
Packaging - Paper ecoinvent 3.6 Database 2019
Supplier data +
Plastic - Plexiglass (PMMA) Product composition + ecoinvent 3.6 2019
database
Plastic - Polyamide ecoinvent 3.6 Database 2019
Plastic - Polycarbonate (PC) ecoinvent 3.6 Database 2019
Rubber, synthetic ecoinvent 3.6 Database 2019
Silicone ecoinvent 3.6 Database 2019
4 / 13
System boundaries (X=included, MND=module not declared, MNR=module not relevant)
Construction Beyond the system
Product stage Use stage End of life stage
installation stage boundaries
A1 A2 A3 A4 A5 B1 B2 B3 B4 B5 B6 B7 C1 C2 C3 C4 D
X X X X X MND MND MND MND MND X MND X X X X X
System boundary:
The analysis is a cradle-to-grave study made for one luminaire manufactured , installed and used in an indoor setting over the lifetime. Modules
A1-A5 are included in the analysis. It includes the extraction and production of raw materials, transportation to the factory, the production process
itself, transportation to market and installation of the product. B6 is the operational energy usage based on a normal use. C1-C4, D are mandatory
modules which include end of life treatment of materials and the benefits from recycling.
Additional technical information:
waR slairetam tropsnarT gnirutcafunaM tropsnarT ylbmessA e​sU ecnanetniaM riapeR tnemecalpeR tnemhsibrufeR lanoitarepO ygrene esu lanoitarepO esu retaw -eD noitcurtsnoc noitilomed tropsnarT etsaW gnissecorp lasopsiD -yrevoceR-esueR laitnetop-gnilcyceR
5 / 13
LCA: Scenarios and additional technical information
The following information describe the scenarios in the different modules of the EPD.
Module A4 = Truck freight from factory to port in China 40 km, sea freight from China to Europe 11 500 km, truck freight from port to
warehouse Norway 20 km, truck freight from warehouse to customer in Norway 300 km.
Modules A5 = No energy use has been quantified since installation in buildings is often done by manual labor. Use of portable electrical devices
(e.g., drill) usually have low energy requirements falling under the cut-off criterion of 1%
Module B6 = The operational energy use of the luminaire is calculated based on the methodology provided in IBU PCR Part B for luminaires,
lamps, and components for luminaires. The energy consumption model for luminaire used in the PCR follows the application scenarios developed
in EN 15193:2007. To calculate the electricity use of the luminaire, the following scenario parameters have been applied:
- Active power of the luminaire (Pa) = 48 watt
- Passive power of the luminaire (Pp) = 0 watt
- Daylight time usage (tD) = 2250 hours
- Non-daylight time usage (tN) = 250 hours
- Standard year time (ty) = 8760 hours
- The occupancy depency factor (FO) = 1 (factor, no unit)
- The daylight dependency factor (FD) = 0.9 (factor, no unit)
- The product specific constant illuminance factor (FCP) = 1 (factor, no unit)
- The non-daylight dimming factor (FN) = 1 (factor, no unit)
- The application specific empiric lifetime of the luminaire in years (a) = 20 years (corresponding to the reference service life of the product).
Module C1 = De-installation of luminaires is often done by manual labor and only in some cases with machines. Energy use is only relevant when
installed with aid from machines. The use of portable electrical devices (e.g., drill) usually have low energy requirements falling under the cut-off
criterion of 1% and can often be neglected.
Module C2 = 85 km is the average default transportation from demolition to waste treatment facility.
Modules C3 and C4 = Waste treatment of the product follows the default values provided in EN 50693, Product Category Rules for life cycle
assessments of electronic and electrical products and systems, table G.4. This table specified how different types of raw materials used in A1 will
likely be treated during the end-of-life of the product. Waste treatments in C3 include material recycling and incineration with and without energy
recovery and fly ash extraction. Disposal in C4 consist of landfilling of different waste fractions and of ashes.
Module D = The recyclability of metals, plastics, and electronic components allows the producers a credit for the net scrap that is produced at the
end of a product’s life. The benefits from recycling of net scrap are described in formula from EN 15804:2012+A2:2019. Substitution of heat and
electricity generated by the incineration with energy recovery of plastic insulation and other parts is also calculated in module D.
Capacity utilisation Value
Transport from production place to user (A4) Distance (km) Fuel/Energy Consumption Unit
(incl. return) % (Liter/tonne)
Ship, Freight, Transoceanic (km) 65,0 % 11500 0,003 l/tkm 34,50
Truck, 16-32 tonnes, EURO 5 (km) - World 38,8 % 40 0,045 l/tkm 1,80
Truck, 16-32 tonnes, EURO 6 (km) - Europe 36,7 % 320 0,043 l/tkm 13,76
Assembly (A5) Unit Value
Waste, packaging, kraft paper, unbleached, to
kg 0,055
average treatment (kg) - A5, inkl. 85 km transp.
Waste, packaging, corrugated board box, 0 %
recycled, to average treatment (kg) - A5 including kg 0,41
transport (kg)
Operational energy (B6) Unit Value
Electricity, Norway (kWh) kWh 1638.00
Capacity utilisation Value
Transport to waste processing (C2) Distance (km) Fuel/Energy Consumption Unit
(incl. return) % (Liter/tonne)
Truck, 16-32 tonnes, EURO 6 (km) - Europe 36,7 % 85 0,043 l/tkm 3,66
6 / 13
Waste processing (C3) Unit Value
Waste treatment per kg used electronic
kg 0,35
components, manual seperation (kg)
Waste treatment of polyvinylchloride (PVC),
incineration with energy recovery and fly ash kg 0,043
extraction (kg)
Steel to recycling (kg) kg 0,12
Non-ferrous metal to recycling (kg) kg 0,00024
Waste treatment of plastic mixture, incineration
kg 0,38
with energy recovery and fly ash extraction (kg)
Aluminium to recycling (kg) kg 0,43
Waste treatment per kg electronics scrap from
LED plate, without components, recycling of kg 0,048
copper - C3 (kg)
Waste treatment per kg used PWB, shredding and kg 0,21
separation - C3 (kg)
Copper to recycling (kg) kg 0,054
Waste treatment of plastic mixture, incineration
kg 0,083
with energy recovery and fly ash extraction (kg)
Waste treatment per kg electronics scrap from
PWB, with components, recycling of metals C3 kg 0,057
(kg)
Waste treatment per kg electronics scrap from
PWB, with components, recycling of metals C3 kg 0,0028
(kg)
Copper to recycling (kg) kg 0,019
Waste treatment per kg used PWB, shredding and
kg 0,0057
separation - C3 (kg)
Disposal (C4) Unit Value
Landfilling of copper (kg) kg 0,036
Landfilling of plastic mixture (kg) kg 0,052
Landfilling of aluminium (kg) kg 0,18
Landfilling of copper (kg) kg 0,012
Landfilling of hazardous waste (kg) kg 0,10
Landfilling of ashes from incineration of Plastic
kg 0,016
mixture, process per kg ashes and residues (kg)
Landfilling of plastic mixture (kg) kg 0,45
Landfilling of ashes from incineration of
Polyvinylchloride (PVC), process per kg ashes and kg 0,0068
residues (kg)
Landfilling of steel (kg) kg 0,030
Landfilling of non-ferrous metal (kg) kg 0,00016
Benefits and loads beyond the system
Unit Value
boundaries (D)
Substitution of primary copper with net scrap (kg) kg 0,054
Substitution of primary aluminium with net scrap
kg 0,43
(kg)
Substitution of electricity, in Norway (MJ) MJ 0,76
Substitution of primary metals with net scrap
kg 0,00084
from PWB, with components (kg)
Substitution of thermal energy, district heating, in
MJ 11,53
Norway (MJ)
Substitution of electricity in Norway (MJ) MJ 0,026
Substitution of primary metals with net scrap
kg 0,016
from PWB, with components (kg)
Substitution of thermal energy, district heating, in
MJ 0,40
Norway (MJ)
Substitution of copper with net scrap from PWB,
kg 0,019
without components (kg)
Substitution of primary other non-ferrous metals
kg 0,00024
with net scrap (kg)
Substitution of primary steel with net scrap (kg) kg 0,12
Substitution of copper with net scrap from PWB,
kg 0,0048
without components (kg)
7 / 13
LCA: Results
The LCA results are presented below for the declared unit defined on page 2 of the EPD document.
Environmental impact
Indicator Unit A1 A2 A3 A4 A5
GWP-total kg CO2 -eq 5,02E+01 4,92E-02 4,02E+00 4,35E-01 6,22E-01
GWP-fossil kg CO2 -eq 5,06E+01 4,91E-02 4,01E+00 4,35E-01 8,18E-03
GWP-biogenic kg CO2 -eq -5,54E-01 1,94E-05 4,08E-03 1,40E-04 6,13E-01
GWP-luluc kg CO2 -eq 9,01E-02 1,78E-05 6,88E-04 2,49E-04 2,60E-06
ODP kg CFC11 -eq 2,68E-06 1,08E-08 3,58E-08 9,44E-08 1,65E-09
AP mol H+ -eq 4,53E-01 1,46E-04 2,11E-02 9,60E-03 4,36E-05
EP-FreshWater kg P -eq 6,08E-03 4,44E-07 8,95E-05 2,42E-06 7,28E-08
EP-Marine kg N -eq 5,55E-02 2,87E-05 4,29E-03 2,34E-03 1,56E-05
EP-Terrestial mol N -eq 6,19E-01 3,21E-04 4,72E-02 2,61E-02 1,68E-04
POCP kg NMVOC -eq 1,99E-01 1,21E-04 1,23E-02 6,88E-03 4,67E-05
ADP-minerals&metals1 kg Sb-eq 5,22E-03 1,33E-06 1,33E-05 6,31E-06 1,87E-07
ADP-fossil1 MJ 5,98E+02 7,30E-01 3,55E+01 5,91E+00 1,11E-01
WDP1 m3 1,77E+03 3,57E-01 9,93E+01 2,79E+00 1,46E-01
Indicator Unit B6 C1 C2 C3 C4 D
GWP-total kg CO2 -eq 3,99E+01 0,00E+00 3,61E-02 1,28E+00 8,71E-02 -5,42E+00
GWP-fossil kg CO2 -eq 3,86E+01 0,00E+00 3,61E-02 1,28E+00 8,69E-02 -5,32E+00
GWP-biogenic kg CO2 -eq 1,07E+00 0,00E+00 1,49E-05 2,30E-04 2,63E-05 -2,20E-02
GWP-luluc kg CO2 -eq 1,59E-01 0,00E+00 1,28E-05 2,20E-04 2,07E-04 -7,78E-02
ODP kg CFC11 -eq 2,65E-06 0,00E+00 8,17E-09 9,99E-09 3,94E-09 -5,04E-03
AP mol H+ -eq 3,02E-01 0,00E+00 1,04E-04 6,28E-04 1,82E-04 -1,26E-01
EP-FreshWater kg P -eq 2,78E-03 0,00E+00 2,88E-07 3,36E-06 1,18E-06 -7,65E-04
EP-Marine kg N -eq 3,32E-02 0,00E+00 2,05E-05 1,88E-04 1,09E-04 -8,36E-03
EP-Terrestial mol N -eq 4,32E-01 0,00E+00 2,29E-04 2,00E-03 5,26E-04 -1,07E-01
POCP kg NMVOC -eq 1,16E-01 0,00E+00 8,79E-05 5,14E-04 2,10E-04 -3,24E-02
ADP-minerals&metals1 kg Sb-eq 2,88E-03 0,00E+00 9,96E-07 8,58E-07 2,06E-07 -1,71E-03
ADP-fossil1 MJ 5,27E+02 0,00E+00 5,45E-01 1,11E+00 4,70E-01 -6,69E+01
WDP1 m3 9,19E+04 0,00E+00 5,27E-01 1,06E+01 3,63E+00 -2,25E+03
GWP-total = Global Warming Potential total; GWP-fossil = Global Warming Potential fossil fuels; GWP-biogenic = Global Warming Potential biogenic; GWP-luluc =
Global Warming Potential land use and land use change; ODP = Depletion potential of the stratospheric ozone layer; AP = Acidification potential, Accumulated
Exceedance; EP-freshwater = Eutrophication potential, fraction of nutrients reaching freshwater end compartment: EP-marine = Eutrophication potential, fraction of
nutrients reaching marine end compartment; EP-terrestrial = Eutrophication potential, Accumulated Exceedance; POCP = Formation potential of tropospheric ozone;
ADP-minerals&metals = Abiotic depletion potential for non-fossil resources; ADP-fossil = Abiotic depletion for fossil resources potential; WDP = Water (user)
deprivation potential, deprivation-weighted water consumption
"Reading example: 9,0 E-03 = 9,0*10-3 = 0,009"
*INA Indicator Not Assessed
1. The results of this environmental impact indicator shall be used with care as the uncertainties on these results are high or as there is limited experienced with the
indicator
Remarks to environmental impacts
8 / 13
Additional environmental impact indicators
Indicator Unit A1 A2 A3 A4 A5
PM Disease incidence 3,15E-06 3,14E-09 2,83E-07 9,56E-09 6,13E-10
IRP2 kgBq U235 -eq 1,41E+00 3,07E-03 3,43E-02 2,55E-02 4,64E-04
ETP-fw1 CTUe 3,03E+03 5,79E-01 1,08E+02 3,83E+00 1,45E-01
HTP-c1 CTUh 7,58E-08 0,00E+00 1,13E-09 0,00E+00 7,00E-12
HTP-nc1 CTUh 3,14E-06 5,83E-10 4,69E-08 1,87E-09 2,63E-10
SQP1 dimensionless 2,03E+02 5,03E-01 7,80E+00 2,10E+00 7,26E-02
Indicator Unit B6 C1 C2 C3 C4 D
PM Disease incidence 2,16E-06 0,00E+00 2,21E-09 3,72E-09 3,32E-09 -5,13E-07
IRP2 kgBq U235 -eq 9,57E+00 0,00E+00 2,38E-03 5,20E-03 1,59E-03 -2,74E-01
ETP-fw1 CTUe 2,40E+03 0,00E+00 4,04E-01 9,23E+00 1,66E+02 -8,51E+02
HTP-c1 CTUh 1,15E-07 0,00E+00 0,00E+00 1,16E-09 1,14E-10 -1,72E-08
HTP-nc1 CTUh 2,70E-06 0,00E+00 4,41E-10 6,82E-08 1,00E-09 -6,43E-07
SQP1 dimensionless 2,66E+02 0,00E+00 3,81E-01 2,54E-01 1,28E+00 -2,11E+01
PM = Particulate Matter emissions; IRP = Ionizing radiation – human health; ETP-fw = Eco toxicity – freshwater; HTP-c = Human toxicity – cancer effects; HTP-nc =
Human toxicity – non cancer effects; SQP = Potential Soil Quality Index (dimensionless)
"Reading example: 9,0 E-03 = 9,0*10-3 = 0,009"
*INA Indicator Not Assessed
1. The results of this environmental impact indicator shall be used with care as the uncertainties on these results are high or as there is limited experienced with the
indicator
2. This impact category deals mainly with the eventual impact of low dose ionizing radiation on human health of the nuclear fuel cycle. It does not consider effects due
to possible nuclear accidents, occupational exposure nor due to radioactive waste disposal in underground facilities. Potential ionizing radiation from the soil, from
radon and from some construction materials is also not measured by this indicator.
9 / 13
Resource use
Indicator Unit A1 A2 A3 A4 A5
PERE MJ 6,64E+01 8,82E-03 1,07E+01 5,66E-02 1,90E-03
PERM MJ 7,37E+00 0,00E+00 0,00E+00 0,00E+00 -7,37E+00
PERT MJ 7,38E+01 8,82E-03 1,07E+01 5,66E-02 -7,37E+00
PENRE MJ 5,71E+02 7,30E-01 3,55E+01 5,91E+00 1,11E-01
PENRM MJ 2,96E+01 0,00E+00 0,00E+00 0,00E+00 0,00E+00
PENRT MJ 6,01E+02 7,30E-01 3,55E+01 5,91E+00 1,11E-01
SM kg 9,96E-02 0,00E+00 0,00E+00 0,00E+00 0,00E+00
RSF MJ 4,02E-01 2,15E-04 7,28E-03 1,70E-03 6,16E-05
NRSF MJ 3,28E-01 1,36E-03 3,56E-02 1,25E-02 3,30E-04
FW m3 4,14E-01 8,07E-05 7,82E-02 4,36E-04 5,69E-05
Indicator Unit B6 C1 C2 C3 C4 D
PERE MJ 6,83E+03 0,00E+00 7,80E-03 1,47E-01 1,08E-01 -2,61E+01
PERM MJ 0,00E+00 0,00E+00 0,00E+00 0,00E+00 0,00E+00 0,00E+00
PERT MJ 6,83E+03 0,00E+00 7,80E-03 1,47E-01 1,08E-01 -2,61E+01
PENRE MJ 5,28E+02 0,00E+00 5,45E-01 1,11E+00 4,70E-01 -6,69E+01
PENRM MJ 0,00E+00 0,00E+00 0,00E+00 -2,96E+01 0,00E+00 0,00E+00
PENRT MJ 5,28E+02 0,00E+00 5,45E-01 -2,85E+01 4,70E-01 -6,69E+01
SM kg 0,00E+00 0,00E+00 0,00E+00 0,00E+00 2,34E-03 3,78E-02
RSF MJ 5,36E+00 0,00E+00 2,79E-04 2,49E-03 5,80E-04 6,76E-05
NRSF MJ 1,34E+01 0,00E+00 9,98E-04 -6,68E-05 2,06E-02 -1,88E-01
FW m3 5,10E+01 0,00E+00 5,83E-05 4,62E-03 4,08E-04 -1,20E-01
PERE = Use of renewable primary energy excluding renewable primary energy resources used as raw materials; PERM = Use of renewable primary energy resources used
as raw materials; PERT = Total use of renewable primary energy resources; PENRE = Use of non renewable primary energy excluding non-renewable primary energy
resources used as raw materials; PENRM = Use of non renewable primary energy resources used as raw materials; PENRT = Total use of non renewable primary energy
resources; SM = Use of secondary materials; RSF = Use of renewable secondary fuels; NRSF = Use of non-renewable secondary fuels; FW = Net use of fresh water
"Reading example: 9,0 E-03 = 9,0*10-3 = 0,009"
*INA Indicator Not Assessed
10 / 13
End of life - Waste
Indicator Unit A1 A2 A3 A4 A5
HWD kg 2,53E-01 5,88E-05 2,12E-02 2,82E-04 0,00E+00
NHWD kg 7,32E+00 3,52E-02 4,56E-01 1,21E-01 4,69E-01
RWD kg 1,16E-03 4,84E-06 2,62E-05 4,07E-05 0,00E+00
Indicator Unit B6 C1 C2 C3 C4 D
HWD kg 3,39E-01 0,00E+00 2,81E-05 3,19E-05 1,19E-01 9,55E-03
NHWD kg 4,06E+01 0,00E+00 2,65E-02 4,32E-02 7,88E-01 -1,48E+00
RWD kg 4,72E-03 0,00E+00 3,71E-06 1,62E-06 1,42E-06 -2,53E-04
HWD = Hazardous waste disposed; NHWD = Non-hazardous waste disposed; RWD = Radioactive waste disposed
"Reading example: 9,0 E-03 = 9,0*10-3 = 0,009"
*INA Indicator Not Assessed
End of life - Output flow
Indicator Unit A1 A2 A3 A4 A5
CRU kg 0,00E+00 0,00E+00 0,00E+00 0,00E+00 0,00E+00
MFR kg 0,00E+00 0,00E+00 1,12E-01 0,00E+00 3,85E-01
MER kg 0,00E+00 0,00E+00 3,01E-02 0,00E+00 5,50E-02
EEE MJ 0,00E+00 0,00E+00 1,88E-02 0,00E+00 6,19E-02
EET MJ 0,00E+00 0,00E+00 2,85E-01 0,00E+00 9,37E-01
Indicator Unit B6 C1 C2 C3 C4 D
CRU kg 0,00E+00 0,00E+00 0,00E+00 0,00E+00 0,00E+00 0,00E+00
MFR kg 0,00E+00 0,00E+00 0,00E+00 6,31E-01 4,58E-05 -1,48E-03
MER kg 0,00E+00 0,00E+00 0,00E+00 5,11E-01 1,12E-06 -1,95E-04
EEE MJ 0,00E+00 0,00E+00 0,00E+00 7,62E-01 7,27E-05 -4,77E-04
EET MJ 0,00E+00 0,00E+00 0,00E+00 1,15E+01 1,10E-03 -7,22E-03
CRU = Components for re-use; MFR = Materials for recycling; MER = Materials for energy recovery; EEE = Exported energy electrical; EET = Exported energy thermal
"Reading example: 9,0 E-03 = 9,0*10-3 = 0,009"
*INA Indicator Not Assessed
Biogenic Carbon Content
Indicator Unit At the factory gate
Biogenic carbon content in product kg C 0,00E+00
Biogenic carbon content in accompanying packaging kg C 2,17E-01
Note: 1 kg biogenic carbon is equivalent to 44/12 kg CO2
11 / 13
Additional requirements
Greenhouse gas emissions from the use of electricity in the manufacturing phase
National production mix from import, low voltage (production of transmission lines, in addition to direct emissions and losses in grid) of applied
electricity for the manufacturing process (A3).
Electricity mix Source Amount Unit
Electricity, China (kWh) ecoinvent 3.6 1102,91 g CO2-eq/kWh
Electricity, Norway (kWh) ecoinvent 3.6 24,33 g CO2-eq/kWh
Dangerous substances
The product contains no substances given by the REACH Candidate list.
Indoor environment
Additional Environmental Information
Additional environmental impact indicators required in NPCR Part A for construction products
Indicator Unit A1 A2 A3 A4 A5
GWPIOBC kg CO2 -eq 5,10E+01 4,92E-02 3,79E+00 4,35E-01 8,18E-03
Indicator Unit B6 C1 C2 C3 C4 D
GWPIOBC kg CO2 -eq 3,98E+01 0,00E+00 3,61E-02 1,28E+00 8,93E-02 -5,24E+00
GWP-IOBC: Global warming potential calculated according to the principle of instantaneous oxidation. In order to increase the transparency of biogenic carbon​
contribution to climate impact, the indicator GWP-IOBC is required as it declares climate impacts calculated according to the principle of instantaneous oxidation.​
GWP-IOBC is also referred to as GWP-GHG in context to Swedish public procurement legislation.
12 / 13
Bibliography
ISO 14025:2010. Environmental labels and declarations - Type III environmental declarations - Principles and procedures. International
Organization for Standardization.
ISO 14044:2006. Environmental management - Life cycle assessment - Requirements and guidelines. International Organization for
Standardization.
EN 15804:2012+A2:2019. Environmental product declaration - Core rules for the product category of construction products. European
Committee for Standardization.
ISO 21930:2017. Sustainability in buildings and civil engineering works - Core rules for environmental product declarations of construction
products. International Organization for Standardization.
EN 50693:2019. Product category rules for life cycle assessments of electronic and electrical products and systems. European Committee for
Standardization.
Ecoinvent v3, 2019. Allocation, cut-off by classification. Swiss Centre of Life Cycle Inventories.
Iversen et al., (2021). eEPD v2021.09, background information for EPD generator tool system verification, LCA.no. Report number: 07.21. System
verification report.
Philis et al., (2022). EPD generator for IBU PCR part B for luminaires, lamps, and components for luminaires, background information for EPD
generator application and LCA data, LCA.no. Report number: 04.22. PCR verification report.
EPD Norway (2022). NPCR Part A: Construction products and services. The Norwegian EPD foundation. Version 2.0 published 24.03.2021.
IBU (2017). PCR part B for luminaires, lampes and components for luminaires. Institut Bauen und Umwelt e.V. Version 1.7, published 30.11.2017.
Program operator and publisher Phone: +47 977 22 020
The Norwegian EPD Foundation e-mail: post@epd-norge.no
Post Box 5250 Majorstuen, 0303 Oslo, Norway web: www.epd-norge.no
Owner of the declaration: Phone:
+47 41560701
Betek Norge AS e-mail:
ok@betek-norge.no
Juraveien 4, 4636 Kristiansand, Norway web:
Author of the Life Cycle Assessment Phone: +47 916 50 916
LCA.no AS e-mail: post@lca.no
Dokka 6A, 1671 Kråkerøy, Norway web: www.lca.no
Developer of EPD generator Phone: +47 916 50 916
LCA.no AS e-mail: post@lca.no
Dokka 6A, 1671 Kråkerøy, Norway web: www.lca.no
ECO Platform web: www.eco-platform.org
ECO Portal web: ECO Portal
13 / 13
