ENVIRONMENTAL PRODUCT DECLARATION
as per ISO 14025 and EN 15804+A1
Owner of the Declaration Kaimann GmbH
Programme holder Institut Bauen und Umwelt e.V. (IBU)
Publisher Institut Bauen und Umwelt e.V. (IBU)
Declaration number EPD-KAI-20200014-IBC1-EN
Issue date 08.06.2020
Valid to 07.06.2025
Kaiflex HFplus s2
Kaimann GmbH
www.ibu-epd.com | https://epd-online.com
Umwelt Produktdeklaration Name des Herstellers – Name des Produkts
1. General Information
Kaimann GmbH Kaiflex HFplus s2
Programme holder Owner of the declaration
IBU – Institut Bauen und Umwelt e.V. Kaimann GmbH
Panoramastr. 1 Hansastraße 2-5
10178 Berlin 33161 Hövelhof
Germany
Declaration number Declared product / declared unit
EPD-KAI-20200014-IBC1-EN 1 m3 insulation material Kaiflex HFplus s2
This declaration is based on the product Scope:
category rules: Product line Kaiflex HFplus s2
Insulating materials made of foam plastics, 06.2017 Thermal insulation material made of flexible
(PCR checked and approved by the SVR) elastomeric foam for technical building equipment and
industrial installations.
Issue date The EPD is performed in agreement with the demands
08.06.2020 of PCR Part A with reference to EN 15804+A1:2013
and PCR Part B: Requirements on the EPD for
insulating materials made of foam plastics.
Valid to
The EPD is based on the average Kaiflex HFplus s2
07.06.2025
production from two different variations produced in
one plant in Germany.
The owner of the declaration shall be liable for the
underlying information and evidence; the IBU shall not
be liable with respect to manufacturer information, life
cycle assessment data and evidences.
The EPD was created according to the specifications
of EN 15804+A1. In the following, the standard will be
simplified as EN 15804.
Verification
The standard EN 15804 serves as the core PCR
Independent verification of the declaration and data
according to ISO 14025:2010
Dipl. Ing. Hans Peters internally x externally
(chairman of Institut Bauen und Umwelt e.V.)
Dr. Alexander Röder Matthias Klingler
(Managing Director Institut Bauen und Umwelt e.V.)) (Independent verifier appointed by SVR)
2. Product
2.1 Product description/Product definition For the application and use the respective national
Kaiflex HFplus s2 is a flexible closed cell rubber provisions apply.
insulation that prevents condensation and reduces
energy loss. By incorporating a water vapour barrier
into the insulation cell structure Kaiflex HFplus s2 can 2.2 Application
effectively eliminate water vapour migration and retain Kaiflex HFplus s2 is available in tube and sheets for
its performance over the entire system life. This EPD use on air-conditioning, refrigeration, chilled water,
covers the Kaiflex HFplus s2 product family including heating and hot water pipes and air-distribution
Kaiflex HFplus s2 tubes and sheets. ductwork. In addition to preventing condensation and
saving energy, Kaiflex HFplus s2 also performs an
For the placing on the market of the product in the acoustic function, absorbing sound and dampening
European Union/European Free Trade Association duct wall vibration. With inherent anti-microbial
(EU/EFTA) (with the exception of Switzerland) resistance as standard, and a Class D fire rated,
Regulation (EU) No. 305/2011 (CPR) applies. The closed cell rubber that is completely dust and fibre
product needs a declaration of performance taking into free, Kaiflex HFplus s2 can be used in any kind of
consideration EN 14304:2009 Thermal insulation public, commercial or industrial building without
products for building equipment and industrial impacting on health or the quality of air. Outdoor
installations - Factory made flexible elastomeric foam application requires protection against UV-radiation.
(FEF) products - Specification, and the CE-marking.
2 Environmental Product Declaration Kaimann GmbH – Kaiflex HFplus s2
2.3 Technical Data which are not on the candidate list, exceeding 0.1
percentage by mass: no.
3) Biocide products were added to this construction
Constructional data product or it has been treated with biocide products
Name Value Unit (this then concerns a treated product as defined by the
Gross density 88 kg/m3 (EU) Ordinance on Biocide Products No. 528/2012):
Water vapour diffusion resistance no.
µ ≥ 2000 -
factor acc. to EN 12088
λϑ = 0.04 + 2.6 Manufacture
8.0 · 10E-5 Upon delivery, the raw materials are either stored in a
Thermal conductivity W/(mK)
ϑ + 7*10E- warehouse or used in the production shortly after. The
7*ϑ² first step in the production of Kaiflex HFplus s2 is to
Thermal conductivity at -10 °C 0.039 W/(mK) mix the raw materials in a kneader and to roll out the
Thermal conductivity at 0 °C 0.04 W/(mK) resulting mixture which is then cut into sheets. The flat
Thermal conductivity at 10 °C 0.041 W/(mK) sheets are passed through an industrial cooler and
cooled off. The cooled-off sheets are granulated and
Performance data of the product in accordance with the granulates are temporarily stored at room
the declaration of performance with respect to its temperature before entering the compounding plant.
essential characteristics according to EN 14304:2009,
Thermal insulation products for building equipment and In a next step, the different types of granulates enter
industrial installations - Factory made flexible the compounding plant for mixing. The resulting
elastomeric foam (FEF) products - Specification. elastomer compound is pushed through one of five
extruders and carried on a conveyer belt through an
industrial furnace for foaming. After foaming, the
endless sheets are passed through an industrial cooler
2.4 Delivery status upon which a continuous longitudinal cut is applied to
The EPD is declared as an average product of one cut sheets into the right width. If applicable, adhesive
plant of one manufacturer. It looks at the average coating is applied on one side of the sheets. Finally, a
environmental performance of six product varieties traverse cut trims the continuous sheet into sheets of
from the product line Kaiflex HFplus s2. This is in various sizes.
accordance with the classification rules for group 1c)
from PCR Part A paragraph 5.2. The products are: 2.7 Environment and health during
manufacturing
The manufacturer of the product complies with national
 Kaiflex HFplus s2 tube
manufacturing guidelines and regulations such as the
 Kaiflex HFplus s2 sheet
German Energy Saving Regulation (EnEV) and the
German Renewable Energy Act (EEG). In addition,
Sheets are available from d = 3 mm to 32 mm. Tubes KAIMANN’s environmental management system is
N
are available from d = 6 mm to 32 mm certified in accordance with ISO 9001/14001/50001.
N
2.5 Base materials/Ancillary materials 2.8 Product processing/Installation
Kaiflex HFplus s2 is based on synthetic rubber and The installation of Kaiflex HFplus s2 requires basic
consists of several components. The following table tools such as cutters and scissors. No additional
shows the components clustered into substance specific protection, beyond normal protective clothes,
groups: is required. Liquid oxygen can react explosively in
conjunction with organic material such as Kaiflex
 Rubber and polymers: 28% HFplus s2 insulation material. To avoid the diffusion of
oxygen, a complete seal must be affected. Butt joints
 Fillers and pigments: 2.6%
and overlapping areas must also be made airtight
 Blowing agent: 7%
using Kaiflex adhesive.
 Vulcanisation system, additives, plasticizer:
12.1% 2.9 Packaging
 Flame retardant: 50% Kaiflex HFplus s2 is packaged in cardboard boxes,
polyethylene film, and polypropylene bags, both in
 Stabilizer: 0.3%
varying sizes. Cardboard boxes and polypropylene
bags are placed on wooden EURO pallets.
Rubber and polymer are the base material. Fillers and
pigments are for firmness and colour. The blowing
agent causes the volume increase and expansion 2.10 Condition of use
process during the manufacture of the product. The Changes in materials composition of the product
vulcanisation system, additives, and plasticizer provide during the use phase only occur in case of
flexibility and workability. The flame retardants ensure extraordinary effects.
the fire resistance of the end-product, and the
adhesives and stabilizers are for processing and 2.11 Environment and health during use
process control. An odour should be considered normal. The odour will
dissipate during use (about 4 weeks) because the cells
1) This product/article/at least one partial article are exchanged with the air.
contains substances listed in the ECHA candidate list
(16.01.2020) exceeding 0.1 percentage by mass: no.
2) This product/article/at least one partial article
contains other CMR substances in categories 1A or 1B
3 Environmental Product Declaration Kaimann GmbH – Kaiflex HFplus s2
2.12 Reference service life Formed from thousands of independently water-
resistant cells, Kaiflex insulation is naturally resistant to
moisture ingress and requires no additional water
Since the use stage (B1-B7) is not fully declared, the vapour barrier.
declaration of the reference service life is only
voluntary. Mechanical destruction
Kaiflex insulation materials are flexible foams and
2.13 Extraordinary effects display limited mechanical rigidity. If the material
should be subjected to mechanical loads, it should be
Fire protected accordingly.
Kaiflex HFplus s2 has been designed to meet
European fire regulations and is a self- extinguishing 2.14 Re-use phase
foam that will not drip, or support flame spread. With a At the end-of-life, the product can be used for energy
European Class DL-s2, d0 or Class D-s2, d0 fire recovery in a waste incineration plat, as well the plastic
classification, Kaiflex HFplus s2 can be used in public, from packaging. The cardboard and wooden pallets
commercial and industrial buildings. from packaging can be recycled.
Fire protection 2.15 Disposal
Name Value The product is disposed in accordance with local
Building material class D (sheets) / DL (tubes) regulations governed by the European Waste
Burning droplets d0 Catalogue (waste code: 07 wastes from organic
Smoke gas development s2 chemical processes - 07 02 13 waste plastic).
Water 2.16 Further information
Additional information about the product is available on
https://kaimann.com/.
3. LCA: Calculation rules
3.1 Declared Unit as well as buildings to manufacture the declared unit,
The declared unit is 1 m³ of the thermal insulation is neglected. On average, 0.49 kWh electricity and
material for technical building equipment and industrial 2.65 kWh natural gas are required for the
installations Kaiflex HFplus s2 including packaging manufacturing of 1m³ Kaiflex HFplus s2. This data was
materials. The declared unit refers to the product as it provided by Kaimann GmbH. This module also
leaves the factory gate. The gross density is the includes packaging with plastics and carboard and
average density of al declared products, weighted by wooden pallets. the biogenic carbon stored is declared
production volume. in the result section.
Module A4: The transport of Kaiflex HFplus s2 from
Declared unit the factory gate to the site of assembly is represented
Name Value Unit through generic background data. The transportation
Gross density 88 kg/m3 distances are based on average transportation data
Conversion factor to 1 kg 88 - provided by the manufacturer.
Declared unit 1 m3 Module A5: The assembly can be done manually
without the use of any electrical equipment. Only glue
(Kaiflex Special glue) is required for the assembly of
Kaiflex HFplus s2. Packaging material from module A3
3.2 System boundary is disposed of here: Plastic packaging is incinerated,
The type of EPD is cradle to gate. The system and cardboard and the wooden pallets are re-used.
boundaries of the EPD follow the modular structure of Modules B1-B7: No resource use and impacts occur
EN 15804 (according to EN 15804, section 6.2.1). Only during the use phase of the products.
the declaration of the product stage modules A1 to A3 Modules C1&C3: Dismantling of Kaiflex HFplus s2 is
is mandatory for compliance with EN 15804. The done manually without using any electrical equipment.
declaration of the modules of other life cycle stages is No processing is required before disposal. Therefore,
optional. Resources from the ecosphere and module C1 and C3 are disregarded.
Technosphere enter the system on stage A1 and leave Module C2: The products to be disposed of are
the system on stage C4. The following life cycle stages transported to the waste treatment facility.
are considered: Module C4: The waste is treated according to the
waste framework directive of the European Union.
Module A1: The system boundaries comprise raw Module D: Potential impacts and benefits from energy
material extraction and supply from cradle to factory recovery and recycling are described.
gate and is represented through generic background
data sets. 3.3 Estimates and assumptions
Module A2: The transport of the raw materials from Module A2: Raw materials are transported to the
the factory gate to the point of manufacturing is manufacturer by road transport and shipping.
represented through generic background data sets. Information on the transportation distances was
The transportation distances have been provided by provided by the manufacturer. For the calculation, the
the manufacturer. distances were weighted by the mass of the respective
Module A3: The manufacturing includes raw materials.
manufacturer-specific material and energy data which
are represented through generic data sets. Machinery,
4 Environmental Product Declaration Kaimann GmbH – Kaiflex HFplus s2
Module A3: No production waste is assumed during
the production of Kaiflex. 3.7 Period under review
The production data refers to the average of the year
Module A4: Kaiflex HFplus s2 is distributed in Europe. 2018.
The average transportation distance per declared unit
was calculated based on the sales volume and 3.8 Allocation
average transportation distance per country where No allocation is carried out.
Kaiflex HFplus s2 is distributed. Based on the sum
product of sales volume multiplied with road 3.9 Comparability
transportation, the total transportation distances were Basically, a comparison or an evaluation of EPD data
calculated and divided by the total sales volume to is only possible if all the data sets to be compared
calculate the average transportation distance per were created according to EN 15804 and the building
declared unit. As a result, the average road context, respectively the product-specific
transportation distance per declared unit is 743 km, characteristics of performance, are taken into account.
and the average ship transportation distance is 97 km.
No loss during transportation is assumed. As a background database GaBi database
professional database (version from September 2019)
Module A5: Kaiflex HFplus s2 is assembled by by thinkstep AG was used and has been
manual labour under use of adhesive. It is assumed complemented by data sets from GaBi extension
that no further energy or materials are required in this databases as well as data sets from the EuGeos
module, and that consumers of Kaiflex HFplus s2 order database 15804-IA database version 2.1 by EuGeos
correct product sizes and thus avoid waste production Ltd.
during the assembly. The packaging materials are
disposed of by re-using (cardboard and wooden pallet)
and by incineration (polyethylene and polypropylene).
Module C2: The average distance of the
disassembled product to the point of disposal is
assumed to be 75 kilometres covered by road.
Module C4: The product is incinerated.
3.4 Cut-off criteria
All material flows in module A1 are covered and almost
all material and energy flows in module A3 are
covered. Neglected material or energy flows have a
mass or energy contribution of less than one percent
per process and contribute to less than 5% of mass
and energy flows of a module. Infrastructure such as
office buildings and the manufacturing hall as well as
the machinery required to produce the product have
not been considered.
3.5 Background data
The LCA model underlying this EPD was created in
openLCA 1.10 developed by GreenDelta GmbH. As a
background database GaBi database professional
database (version from September 2019) by thinkstep
AG was used and has been complemented by data
sets from GaBi database extension databases as well
as data sets from the EuGeos database 15804-IA
database version 2.1 by EuGeos Ltd.
3.6 Data quality
The life cycle inventory for the assessed product is
based on an internal assessment of manufacturing and
environmental data, assessment of LCA-relevant data
for the supply chain and energy measurement within
the factors. The required product flows for creation of
the product system were handed over to GreenDelta
GmbH.
All data was scrutinised and found to be plausible and
consistent and were therefore found to be
representative.
Some of the background data sets are more than 10
years old but were used when no recent dataset was
available. Datasets from the GaBi database are
assumed to have a high quality.
There are no materials or processes that are left out
because they are under the cut-off threshold.
5 Environmental Product Declaration Kaimann GmbH – Kaiflex HFplus s2
4. LCA: Scenarios and additional technical information
The following technical scenario information serves as
a basis for the declared modules. All values refer to the
declared unit of 1 m³.
Transport to the building site (A4)
Name Value Unit
Transport distance (road) 743 km
transport distance (ship) 97 km
Installation into the building (A5)
Name Value Unit
Auxiliary 1.6 kg
Water consumption 0 m3
Other resources 0 kg
Electricity consumption 0 kWh
Other energy carriers 0 MJ
Material loss 0 kg
Output substances following
16.5 kg
waste treatment on site
Dust in the air 0 kg
VOC in the air 0 kg
The 16.5 kg are the sum of all packaging materials per
declared unit.
End of life (C1-C4)
Name Value Unit
Collected separately 89.6 kg
Collected as mixed construction
0 kg
waste
Reuse 0 kg
Recycling 0 kg
Energy recovery 89.6 kg
Landfilling 0 kg
88 kg Kaiflex and 1.6 kg special glue are incinerated
for energy recovery.
Reuse, recovery and/or recycling potentials (D),
relevant scenario information
Module D includes the credits of the incineration
processes from modules C4 and A5 (packaging waste)
at a waste incineration plant with an assumed
efficiency of R1<0.6.
6 Environmental Product Declaration Kaimann GmbH – Kaiflex HFplus s2
5. LCA: Results
The life cycle impact assessment method is based on EN15804. Energy indicators for resource use utilise the
lower calorific value.
DESCRIPTION OF THE SYSTEM BOUNDARY (X = INCLUDED IN LCA; MND = MODULE NOT DECLARED;
MNR = MODULE NOT RELEVANT)
BENEFITS AND
CONSTRUCTI LOADS
PRODUCT STAGE ON PROCESS USE STAGE END OF LIFE STAGE BEYOND THE
STAGE SYSTEM
BOUNDARIES
7 Environmental Product Declaration Kaimann GmbH – Kaiflex HFplus s2
lairetam
waR
ylppus tropsnarT
gnirutcafunaM
eht
morf
tropsnarT
etis
eht
ot
etag
ylbmessA esU
ecnanetniaM
riapeR
tnemecalpeR tnemhsibrufeR
ygrene
lanoitarepO esu
retaw
lanoitarepO esu
noitcurtsnoc-eD
noitilomed tropsnarT
gnissecorp
etsaW
lasopsiD -esueR -yrevoceR -gnilcyceR laitnetop
A1 A2 A3 A4 A5 B1 B2 B3 B4 B5 B6 B7 C1 C2 C3 C4 D
X X X X X MND MND MNR MNR MNR MND MND MND X MND X X
RESULTS OF THE LCA - ENVIRONMENTAL IMPACT according to EN 15804+A1: 1 m³
Parameter Unit A1 A2 A3 A4 A5 C2 C4 D
GWP [kg CO2-Eq.] 2.84E+2 6.64E+0 2.64E+1 1.08E+1 1.27E+1 1.08E+0 2.27E+2 -2.44E+2
ODP [kg CFC11-Eq.] 4.77E-5 7.57E-7 2.23E-7 1.99E-6 2.88E-7 2.01E-7 1.56E-13 -2.23E-7
AP [kg SO2-Eq.] 1.35E+0 8.98E-2 8.69E-2 4.57E-2 1.74E-2 4.26E-3 2.57E-2 -2.33E-1
EP [kg (PO4)3--Eq.] 2.18E+0 1.17E-2 2.05E-2 1.03E-2 8.10E-3 1.00E-3 5.99E-3 -5.54E-2
POCP [kg ethene-Eq.] 6.59E-2 2.72E-3 5.07E-3 1.86E-3 2.36E-3 1.78E-4 1.51E-3 -1.19E-2
ADPE [kg Sb-Eq.] 1.53E-3 1.23E-5 9.33E-6 3.21E-5 1.15E-5 3.24E-6 1.52E-6 -1.35E-5
ADPF [MJ] 4.90E+3 9.41E+1 3.19E+2 1.67E+2 1.08E+2 1.67E+1 9.43E+1 -1.89E+3
GWP = Global warming potential; ODP = Depletion potential of the stratospheric ozone layer; AP = Acidification potential of land and water; EP =
Caption Eutrophication potential; POCP = Formation potential of tropospheric ozone photochemical oxidants; ADPE = Abiotic depletion potential for non-
fossil resources; ADPF = Abiotic depletion potential for fossil resources
RESULTS OF THE LCA - RESOURCE USE according to EN 15804+A1: 1 m³
Parameter Unit A1 A2 A3 A4 A5 C2 C4 D
PERE [MJ] 3.08E+2 7.75E-1 2.79E+2 1.79E+0 7.93E+0 1.80E-1 2.64E+1 -5.58E+2
PERM [MJ] 7.94E+0 0.00E+0 2.35E+2 0.00E+0 0.00E+0 0.00E+0 0.00E+0 -2.35E+2
PERT [MJ] 3.16E+2 7.75E-1 5.13E+2 1.79E+0 7.93E+0 1.80E-1 2.64E+1 -7.93E+2
PENRE [MJ] 1.45E+3 9.51E+1 2.24E+2 1.69E+2 2.26E+2 1.69E+1 3.83E+3 -1.89E+3
PENRM [MJ] 3.73E+3 0.00E+0 1.16E+2 0.00E+0 -1.16E+2 0.00E+0 -3.73E+3 0.00E+0
PENRT [MJ] 5.18E+3 9.51E+1 3.40E+2 1.69E+2 1.10E+2 1.69E+1 9.43E+1 -1.89E+3
SM [kg] 0.00E+0 0.00E+0 0.00E+0 0.00E+0 0.00E+0 0.00E+0 0.00E+0 0.00E+0
RSF [MJ] 0.00E+0 0.00E+0 0.00E+0 0.00E+0 0.00E+0 0.00E+0 0.00E+0 0.00E+0
NRSF [MJ] 0.00E+0 0.00E+0 0.00E+0 0.00E+0 0.00E+0 0.00E+0 0.00E+0 0.00E+0
FW [m³] 6.11E+0 1.23E-2 7.24E-1 2.83E-2 2.27E-1 2.85E-3 7.39E-1 -4.31E+0
PERE = Use of renewable primary energy excluding renewable primary energy resources used as raw materials; PERM = Use of
renewable primary energy resources used as raw materials; PERT = Total use of renewable primary energy resources; PENRE = Use of
non-renewable primary energy excluding non-renewable primary energy resources used as raw materials; PENRM = Use of non-
Caption
renewable primary energy resources used as raw materials; PENRT = Total use of non-renewable primary energy resources; SM = Use
of secondary material; RSF = Use of renewable secondary fuels; NRSF = Use of non-renewable secondary fuels; FW = Use of net fresh
water
RESULTS OF THE LCA – OUTPUT FLOWS AND WASTE CATEGORIES according to EN 15804+A1:
1 m³
Parameter Unit A1 A2 A3 A4 A5 C2 C4 D
HWD [kg] 3.49E-2 3.37E-9 9.50E-3 1.60E-10 4.35E-8 0.00E+0 5.84E-7 -1.71E-3
NHWD [kg] 1.58E+2 6.61E-2 9.01E+0 3.13E-3 4.54E+0 0.00E+0 6.65E+1 -3.54E+2
RWD [kg] 3.86E-2 3.77E-5 2.79E-3 1.79E-6 8.02E-4 0.00E+0 4.52E-3 -5.17E-3
CRU [kg] 0.00E+0 0.00E+0 0.00E+0 0.00E+0 1.37E+1 0.00E+0 0.00E+0 0.00E+0
MFR [kg] 0.00E+0 0.00E+0 0.00E+0 0.00E+0 0.00E+0 0.00E+0 0.00E+0 0.00E+0
MER [kg] 5.55E-11 0.00E+0 0.00E+0 0.00E+0 0.00E+0 0.00E+0 0.00E+0 0.00E+0
EEE [MJ] 0.00E+0 0.00E+0 0.00E+0 0.00E+0 0.00E+0 0.00E+0 0.00E+0 0.00E+0
EET [MJ] 0.00E+0 0.00E+0 0.00E+0 0.00E+0 6.94E+1 0.00E+0 2.24E+3 0.00E+0
HWD = Hazardous waste disposed; NHWD = Non-hazardous waste disposed; RWD = Radioactive waste disposed; CRU = Components
Caption for re-use; MFR = Materials for recycling; MER = Materials for energy recovery; EEE = Exported electrical energy; EEE = Exported
thermal energy
Additional Technical scenario:
Biogenic carbon is not included in the results. It enters the product system with wood and cardboard in modules
A3 and is ‘released’ by being an avoided burden in module A5 (declared in module D) and has thus no net-effect
on the overall results. The wooden pallet has approximately 23 kg biogenic CO2, and the carboard has 16 kg.
6. LCA: Interpretation
Environmental Impacts
The production of the blowing agent uses the most
fresh water.
All seven environmental impact categories are
dominated by module A1 raw material supply. The Hazardous waste disposed (HWD)
production of the blowing agent and the base material Most of the hazardous waste comes from the
are the largest contributors. For the global warming production of the blowing agent in A1 and the
potential, the incineration of the product in module C4 production of the plastic packaging in A3.
is another major source of greenhouse gas emissions.
Non-hazardous waste disposed (NHWD)
Renewable primary energy as energy carrier This impact category is dominated by module A1 raw
(PERE) material supply and the incineration residues in module
Renewable energy is used in the production of the raw C4.
materials and in the production of the packaging The main contributor is the production of the base
(mainly the wooden pallet). Likewise, energy is material.
released in the incineration process (D).
Radioactive waste disposed (RWD)
Renewable primary energy resources as material This impact category is dominated by module A1 raw
utilization (PERM) material supply.
The wood of the pallet acts as a storage for renewable Most radioactive waste stems from the production of
energy. By re-using the pallet, the same amount of the base material.
energy is credited in module D.
Conclusion
Use of net fresh water (FW) The production of the blowing agent is the largest
This impact category is dominated by module A1 raw contributor to the environmental impacts of Kaiflex
material supply. HFplus s2.
7. Requisite evidence
VOC without NIK <5 μg/m3
7.1 VOC emissions Carcinogenic Substances <1 μg/m3
The Volatile Organic Compound (VOC) emissions
have been tested by Eurofins Product Testing A/S by AgBB overview of results (3 days [µg/m³])
using the Committee for health-related evaluation of Name Value Unit
building products/Deutsches Institut für Bautechnik TVOC (C6 - C16) <5 μg/m3
(AgBB/DIBt) test method in 09.2013. Sum SVOC (C16 - C22) <5 μg/m3
R (dimensionless) <1 -
AgBB overview of results (28 days [µg/m³]) VOC without NIK <5 μg/m3
Name Value Unit Carcinogenic Substances <1 μg/m3
TVOC (C6 - C16) <5 μg/m3
Sum SVOC (C16 - C22) <5 μg/m3
7.2 Leaching performance
R (dimensionless) <1 -
8 Environmental Product Declaration Kaimann GmbH – Kaiflex HFplus s2
The concentration of water-soluble chloride ions is 300
mg/kg according to /EN 13468:2001/.
8. References
AGBB/DIBt
Deusches Institut für Bautechnik 2018: Anforderungen ISO 9001
an die Innenraumluftqualität in Gebäuden: ISO 9001:2015, Quality management systems -
Gesundheitliche Bewertung der Emissionen von Requirements
flüchtigen organischen Verbindungen (VVOC, VOC
und SVOC) aus Bauprodukten ISO 14001
ISO 14001:2015-0/, Environmental management
EN 12088 systems - Requirements with guidance for use
EN 12088:2013, Thermal insulating products for
building applications. Determination of long term water ISO 50001
absorption by diffusion ISO 50001:2018-08, Energy management systems -
Requirements with guidance for use
EN 13468
EN 13468:2001, Thermal insulating products for openLCA 1.10
building equipment and industrial installations - open LCA 1.10.2 (2020), Sustainability Software,
Determination of trace quantities of water soluble Databases, and Consulting. Developed by GreenDelta
chloride, fluoride, silicate, and sodium ions and pH GmbH. http://www.openlca.org/
EN 14304 PCR Part A
EN 14304:2009+A1:2013, Thermal insulation products PCR Part A Version 1.8, Calculation Rules for the Life
for building equipment and industrial installations - Cycle Assessment and Requirements on the Project
Factory made flexible elastomeric foam (FEF) Report
products - Specification
PCR Part B
EN 15804 PCR Part B Version 1.6, Requirements on the EPD for
EN 15804:2012+A1:2013, Nachhaltigkeit von insulating materials made of foam plastics
Bauwerken – Umweltproduktdeklarationen –
Grundregeln für die Produktkategorie Bauprodukte REACH 2006
REGULATION (EC) No 1907/2006 OF THE
EuGeos database EUROPEAN PARLIAMENT AND OF THE COUNCIL
LCA database by EuGeos Limited concerning the Registration, Evaluation, Authorisation
and Restriction of Chemicals (REACH)
Eurofins
Eurofins Product Testing A/S, Galten, Denmark SVHC 2019
Candidate List of substances of very high concern for
European waste catalogue 2014 Authorisation (SVHC), European Chemicals Agency,
COMMISSION DECISION amending Decision Helsinki, Finland
2000/532/EC on the list of waste pursuant to Directive
2008/98/EC of the European Parliament and of the thinkstep AG
Council Sustainability Software, Data and Consulting
GABI database
LCA database SP 39. thinkstep AG. Echterdingen
2019
9 Environmental Product Declaration Kaimann GmbH – Kaiflex HFplus s2
Publisher
Institut Bauen und Umwelt e.V. Tel +49 (0)30 3087748- 0
Panoramastr. 1 Fax +49 (0)30 3087748- 29
10178 Berlin Mail info@ibu-epd.com
Germany Web www.ibu-epd.com
Programme holder
Institut Bauen und Umwelt e.V. Tel +49 (0)30 - 3087748- 0
Panoramastr 1 Fax +49 (0)30 – 3087748 - 29
10178 Berlin Mail info@ibu-epd.com
Germany Web www.ibu-epd.com
Author of the Life Cycle
Assessment Tel +49 30 6292 4320
GreenDelta GmbH Fax -
Kaiserdamm 13 Mail gd@greendelta.com
14057 Berlin Web https://www.greendelta.com
Germany
Owner of the Declaration
Kaimann GmbH Tel +49 5257 98 50 - 0
Hansastraße 2-5 Fax +49 5257 98 50 590
33161 Hövelhof Mail info@kaimann.de
Germany Web https://www.kaimann.com
