ENVIRONMENTAL PRODUCT DECLARATION
as per ISO 14025 and EN 15804+A2
Owner of the Declaration voestalpine AG
Publisher Institut Bauen und Umwelt e.V. (IBU)
Programme holder Institut Bauen und Umwelt e.V. (IBU)
Declaration number EPD-VOE-20230106-IBC2-EN
Issue date 09.05.2023
Valid to 08.05.2028
Drawn Wire – Cold Heading Wire
voestalpine Wire Austria GmbH
www.ibu-epd.com | https://epd-online.com
1. General Information
voestalpine Wire Austria GmbH Drawn Wire – Cold Heading Wire
Programme holder Owner of the declaration
IBU – Institut Bauen und Umwelt e.V. voestalpine AG
Hegelplatz 1 voestalpine­Straße 3
10117 Berlin 4020 Linz
Germany Austria
Declaration number Declared product / declared unit
EPD­VOE­20230106­IBC2­EN 1 tonne of CHQ steel­, bearing steel­, spring steel wire
This declaration is based on the product category rules: Scope:
Structural steels, 01.08.2021 This EPD is based on a declared unit of 1 metric tonne of average
(PCR checked and approved by the SVR) voestalpine cold heading (CHQ)­, bearing­, spring steel wire produced at
the production site in Bruck a.d. Mur (Austria).
Issue date The owner of the declaration shall be liable for the underlying information
and evidence; the IBU shall not be liable with respect to manufacturer
09.05.2023
information, life cycle assessment data and evidences.
The EPD was created according to the specifications of EN 15804+A2. In
Valid to
the following, the standard will be simplified as EN 15804.
08.05.2028
Verification
The standard EN 15804 serves as the core PCR
Independent verification of the declaration and data according to ISO
14025:2011
internally X externally
Dipl.­Ing. Hans Peters
(Chairman of Institut Bauen und Umwelt e.V.)
Florian Pronold Prof. Dr. Birgit Grahl,
(Managing Director Institut Bauen und Umwelt e.V.) (Independent verifier)
1 Environmental Product Declaration ­ voestalpine Wire Austria GmbH ­ Drawn Wire – Cold Heading Wire
2. Product
2.1 Product description/Product definition 2.3 Technical Data
Cold heading wires (CHQ) are used to produce parts of This EPD applies to all cold heading­, bearing and spring steel
complex shapes by means of cold forming operations, using wires from voestalpine Wire Austria GmbH, which is why a
different production techniques, such as cutting, heading, general statement about mechanical parameters is not
upsetting, extrusion or rolling. This kind of forming processes possible. The technical data given for the products are generic
can also be complemented by different machining operations, literature data for steel as described e.g. in Key to Steel. No
such as turning, grinding, polishing and others. product specific test rules are applicable to the data given:
Bearing steel wires are part of the voestalpine Wire Austria Constructional data
GmbH product range. The properties of these wires are
optimized to produce ball­, roller­, cylindrical­ and needle
bearings. Generally, bearing steels are characterized by good
hardenability and high surface hardness, which results in little
material abrasion during use.
Spring steel wires are also a part of the voestalpine Wire
Austria GmbH product range and are used to produce steel
springs. Thanks to optimized alloying concepts and processing
parameters, spring steel is characterized by its high yield
strength to tensile strength ratio, compared to other types of
Various steel grades are processed at the drawing facility of
steel. Therefore, spring steels can be subjected to high loads
voestalpine Wire Austria GmbH.
without plastic deformation.
Cold heading wire steel grades:
In order to fulfill certain requirements concerning mechanical
properties and deformability, specific chemical compositions, as
well as optimized production processes are used to produce
cold heading­, bearing steel­ and spring steel wires.
To ensure high­quality standards, all products are
manufactured under optimized process conditions, such as:
• High degree of purity
• Low core segregation
• Optimized annealing conditions
• Continuous quality inspections and several special
testing options
• End­to­end traceability of all production and test
parameters
• Greatest possible flexibility as the result of an integrated
production chain
• Strict adherence to schedules, and partnerships with our
customers
• Technical and sales service
For the use and application of the product the respective
national provisions at the place of use apply, in Germany for
example the building codes of the federal states and the
corresponding national specifications.
2.2 Application
Cold heading wire products from voestalpine Wire Austria
GmbH are used to produce a variety of components ranging
from safety parts, fasteners, fixations, chains, bolts and rivets to
ball studs and gear wheels.
Special products include cold heading wire for high­strength
screws and highly loaded shafts for automotive lightweight
construction.
Bearing steel wire products from voestalpine Wire Austria
GmbH are used in a wide variety of bearing concepts, such as
ball­, roller­, cylindrical­ or needle bearings.
Spring steel wire products from voestalpine Wire Austria GmbH
are characterized by a high yield strength to tensile strength
ratio and are therefore well suited to produce a wide variety of
spring elements.
2 Environmental Product Declaration ­ voestalpine Wire Austria GmbH ­ Drawn Wire – Cold Heading Wire
selection from the voestalpine Wire Austria GmbH product
range.
Customer­specific changes to the alloy composition can occur
on request.
Performance data of the product with respect to its
characteristics in accordance with the relevant technical
provision (no CE­marking).
2.4 Delivery status
By applying the EN 10278 standard, tightest diameter
tolerances are guaranteed (h8, h9, h10, h11) for all types of
wire products. Cold heading wires produced have a standard
diameter range between 0.8 and 30 mm. Spring wires
according to EN 10270-1 are produced in a dimension range
between 14 and 20 mm. Spring wires according to EN 10089
are produced in a dimension range between 1 and 29 mm.
Bearing wires produced have a standard diameter range
between 1.05 and 26 mm. In terms of surface finish, a
distinction is made between:
• phosphate­free
• end phosphate coated, with a soap or lime coating
• bright drawn
All produced wires are supplied in coils with different coil types:
• catch weight coils
• on carriers
• coreless coils (with/without longitudinal winding,
with/without conical winding)
The outer diameter and weight of the coils vary between 450 to
1500 mm and 350 to 1500 kg, depending on the wire diameter.
2.5 Base materials/Ancillary materials
The starting product for cold heading wire is hot­rolled wire,
which is produced at the voestalpine Wire Rod Austria site. The
basic material for this is in turn crude steel, which consists of
about 85 % pig iron and about 15 % scrap and alloying
elements.
This product/article/at least one partial article contains
substances listed in the candidate list (date: 16.1.2020)
exceeding 0.1 percentage by mass: no.
Further steel grades can be processed on request.
This product/article/at least one partial article contains other
Bearing wire steel grades: carcinogenic, mutagenic, reprotoxic (CMR) substances in
categories 1A or 1B which are not on the candidate list,
exceeding 0.1 percentage by mass: no.
Biocide products were added to this construction product or it
has been treated with biocide products (this then concerns a
treated product as defined by the (EU) Ordinance on Biocide
Products No. 528/2012): no.
Customer­specific changes to the alloy composition can occur 2.6 Manufacture
on request.
The starting material to produce cold heading­, bearing steel­
and spring steel wires is low alloyed steel, which is mainly
Spring wire steel grades:
produced at voestalpine Stahl Donawitz GmbH via the primary
Steels according to EN 10270-1 and EN 10089 are used to
route (blast furnace, LD steel mill, ladle furnace). The steel is
produce drawn spring steel wire. The following alloys are
cast into blooms using a continuous casting process.
suitable to produce quenched and tempered springs and are a
3 Environmental Product Declaration ­ voestalpine Wire Austria GmbH ­ Drawn Wire – Cold Heading Wire
In a further step, the blooms are rolled to the desired dimension The declared product is delivered on wooden pallets. Pallets
in the wire rod rolling mill of voestalpine Wire Rod Austria treated according to the ISPM 15 standard are used on
GmbH. The diameters of the rolled wire rod vary between 5 and customer request. The packaging of the drawn wires varies
31 mm. After the rolling process, the wires are delivered by train according to customer requirements, therefore various
to voestalpine Wire Austria GmbH in Bruck an der Mur. packaging materials are used to protect the wires from
environmental influences, e.g.:
In a first step, the wire rods are pickled in hydrochloric acid. At
• PE (polyethylene) stretch foil
the drawing facility of voestalpine Wire Austria GmbH the wires
• LDPE (low­density polyethylene) foil
are further processed according to EN 10263 specifications.
• VCI (volatile chemical inhibitors) foil
• crepe paper
• cardboard boxes
• wooden boxes
2.10 Condition of use
There is no change in material composition over the service life
of the product. If used as intended, no effects on the
environment are to be expected.
2.11 Environment and health during use
During the use of steel wire products, no effects on human and
animal health and no harmful emissions to air, soil and water
are expected.
2.12 Reference service life
Due to the variety of applications and their stresses,
voestalpine Wire Austria GmbH does not specify a reference
service life for their wire products. Corrosive atmospheres must
be avoided to guarantee a full lifetime of functionality.
2.13 Extraordinary effects
Fire
Steel wires are not flammable, therefore no flammable gases or
The annealing of the coils takes place in a bell­type annealing vapours escape.
furnace at temperatures and times of around 700 °C and 12
hours. Water
No negative consequences for the environment are to be
2.7 Environment and health during manufacturing
expected under the influence of water.
The voestalpine Wire Austria site is certified according to EMAS
III, ISO 9001, ISO 50001 and ISO 14001. As part of the
Mechanical destruction
environmental declarations required by EMAS, voestalpine
Unpredictable mechanical impact on the declared products has
continuously publishes environmentally relevant data and facts
no negative consequences on the environment due to the
about the site.
plastic deformability of steel.
At the Bruck/Mur site, investments are constantly being made in 2.14 Re-use phase
the expansion of environmental protection measures in order to The declared products from voestalpine Wire Austria GmbH
be able to reduce emissions to air and water to a minimum. consist of almost 100 % steel and can therefore be reused or
recycled in the steel industry as a secondary raw material.
All operating facilities that have been approved in accordance
with the environmental impact assessment procedure are also 2.15 Disposal
periodically inspected by the authorities as part of The declared product can be fully used as a recycling raw
environmental inspections. material. The waste code according to the European Waste
Catalogue is: 17 04 05 (iron and steel). The waste type is
2.8 Product processing/Installation
equivalent to the key number 35103 according to the nationally
Drawn wire products from voestalpine Wire Austria GmbH are applicable Waste Catalogue by­law.
processed by a broad range of different customers in the
respective factories. Depending on the desired wire 2.16 Further information
specification, the wire is further processed in different ways, Further information on the product is available on the website at
e.g. cold heading, turning or spring coiling. https://www.voestalpine.com/wiretechnology/en/drawn­wire
2.9 Packaging
3. LCA: Calculation rules
Name Value Unit
3.1 Declared Unit
Declared unit 1 t
This environmental product declaration refers to a declared unit
of 1 tonne of average CHQ­, bearing­, spring steel – automotive
Density 7850 kg/m3
wire. For the calculation of the declared average, input and
Declared unit production quantities for the entire calendar year 2018 were
taken into account and broken down to the declared product
4 Environmental Product Declaration ­ voestalpine Wire Austria GmbH ­ Drawn Wire – Cold Heading Wire
group. The calculated results can thus be considered assumptions from average data (when available) or with
representative for the declared product portfolio of CHQ­, generic data and are documented accordingly. Only data with a
bearing­, spring steel – automotive wire of voestalpine Wire contribution of less than 1 % were cut off. Ignoring such data is
Austria GmbH. justified based on the irrelevance of the expected effect.
Processes, materials, or emissions known to make a significant
A linear correlation of the environmental impacts with the contribution to the environmental effects of the products under
product weight is to be expected. Therefore, the conversion examination have not been neglected. All relevant data were
from the declared unit to a specific product is possible using a collected comprehensively. It is assumed that the data have
mass­specific scaling factor. been completely recorded and the overall total of ignored input
flows do not amount to more than 5 % of total energy and mass
3.2 System boundary flows.
The life cycle assessment of average CHQ­, bearing­, spring Environmental impacts of machines, plant and infrastructure
steel – automotive wire refers to a cradle­to­gate analysis with were not included.
modules (A1–A3 + C +D). Subsequent life cycle phases are
part of the analysis: 3.5 Background data
This study uses generic background data for the evaluation of
Module A1–A3 | Production stage upstream environmental impacts from GaBi­database 2021.1
The production stage includes the burdens of the production of and is modelled in GaBi­­software version 10.
CHQ­, bearing­, spring steel – automotive wire of voestalpine
Wire Austria GmbH at the production site in Bruck a.d. Mur. 3.6 Data quality
Most of the used steel wire is provided by the voestalpine Wire The foreground data collected at voestalpine Wire Austria
Rod Austria from St. Peter Freienstein. Thus, the upstream GmbH are based on the quantities used and volumes produced
environmental impact of the steel supplied is represented by annually. Process data were collected by voestalpine in the
primary data of the respective production site. Material and course of reporting to official agencies. Data on material and
energy flows for the pickling, drawing, cold rolling and energy use originate from material­specific throughput
annealing are considered. Electricity at Bruck a. d. Mur is measurements of various processes as well as from controlling.
provided from 100 % renewable energy (emission factor GWP­ The technological, geographical and time­related
total: 14 g CO ­equivalents/kWh). Thermal energy provision is representativeness of the data base was kept in mind when
2
selecting background data. Whenever specific data were
based on natural gas. Module A1–A3 also includes the
missing, either generic datasets or representative average data
production of the packaging.
were used instead. The implemented GaBi background
datasets are not more than ten years old.
Module C1 | Deconstruction and demolition
It is assumed that the product is not connected with other
3.7 Period under review
materials and can therefore be dismantled. Associated efforts
Foreground data were collected in the 2018 production year,
are negligible, no environmental impacts from the
and the data are based on the volumes produced on an annual
deconstruction of the products are declared.
basis.
Module C2 | Transport 3.8 Geographic Representativeness
The transport to the disposal of the material is estimated
Land or region, in which the declared product system is
declaring a 50 km radius to the waste processing.
manufactured, used or handled at the end of the product´s
lifespan: Austria
Module C3 | Waste processing
Product flows that reach Module D for recycling leave the
product system in C3. Environmental impacts resulting from the 3.9 Allocation
grinding and sorting of steel scrap are not included due to the The primary data for the upstream production of the steel billets
negligible expected environmental impact. were allocated using the partitioning approach developed by
worldsteel 2014 for calculating life cycle inventories of co­
Module C4 | Landfilling products in steel production, which is in line with the provisions
Module C4 declares the environmental impacts incurred by of EN 15804. The so­called partitioning approach provides for
landfilling (5 % of the product). the allocation of environmental effects on the steelmaking
process and the emerging byproducts based on physical
Module D | Benefits and loads beyond the system relations. Material­inherent flow properties are, thus, taken into
boundary account.
The potential for substituting primary steel with a recycling
scenario (95 % of the product) is outlined in Module D. Economic allocation is not considered as referring byproducts
and co­products are not directly tradable goods. Furthermore,
3.3 Estimates and assumptions
long­term contracts for the sale of the byproducts exist, and the
All assumptions are verified through detailed documentation
negotiated prices are, therefore, not subject to market
and correspond to the best possible representation of reality
dynamics.
based on the available data. Regional applicability of the used
background data refers to average data under European or 3.10 Comparability
German conditions taken from the GaBi­database. German Basically, a comparison or an evaluation of EPD data is only
data were used for the Austrian market whenever European or possible if all the data sets to be compared were created
Austrian average data were not available. according to EN 15804 and the building context, respectively
the product­specific characteristics of performance, are taken
3.4 Cut-off criteria
into account. The GaBi background database was used to
All inputs and outputs for which data are available are included
calculate the LCA (GaBi 10; 2021.1).
in the LCA model. Data gaps are filled with conservative
5 Environmental Product Declaration ­ voestalpine Wire Austria GmbH ­ Drawn Wire – Cold Heading Wire
4. LCA: Scenarios and additional technical information
The end­of­life scenario used in this LCA study is based on the
Characteristic product properties of biogenic carbon following assumptions and thus complies with the specifications
The declared product does not contain any biogenic carbon. published in ökobaudat 2022:
Information on describing the biogenic Carbon Content at End of life (C1–C4)
factory gate
Name Value Unit
Name ValueUnit
Collected separately (steel) 1000 kg
Biogenic carbon content in accompanying kg
3.75 Recycling 95 % 950 kg
packaging C
Landfilling 5 % 50 kg
The carbon stored in the packaging was taken into account as
"CO ­neutral". Thus the storage effect of the carbon bound in Reuse, recovery and/or recycling potentials (D), relevant
2
scenario information
the packaging is not included in the calculation but is
considered as emitted immediately. Name Value Unit
Net flow of steel scrap 856 kg
This scenario contains a recycling rate of 95 %. Since
voestalpine externally purchases scrap for steel production, this
is offset against the steel scrap for recycling (net flow).
Installation into the building (A5)
The end­of­life of the packaging materials is not declared in
Module A5.
Name Value Unit
Packaging (binding wire, packaging strips) 1.2 kg
Packaging (plastic) 0.1 kg
Packaging (cardboard) 0.08 kg
Packaging (wood) 8.3 kg
6 Environmental Product Declaration ­ voestalpine Wire Austria GmbH ­ Drawn Wire – Cold Heading Wire
5. LCA: Results
The following table contains the LCA results for a declared unit of 1 tonne of CHQ­, bearing­, spring steel – automotive wire.
DESCRIPTION OF THE SYSTEM BOUNDARY (X = INCLUDED IN LCA; ND = MODULE OR INDICATOR NOT DECLARED; MNR =
MODULE NOT RELEVANT)
Benefits and
Construction loads beyond
Product stage Use stage End of life stage
process stage the system
boundaries
la ire ta m w a Ry lp p u s tro p s n a rT g n iru tc a fu n a M e h t m o rf tro p s n a rTe tis e h t o t e ta g y lb m e s s A e s U e c n a n e tn ia M ria p e R tn e m e c a lp e R tn e m h s ib ru fe R y g re n e la n o ita re p Oe s u re ta w la n o ita re p Oe s u n o itc u rts n o c ­e Dn o itilo m e d tro p s n a rT g n is s e c o rp e ts a W la s o p s iD ­e s u e R­y re v o c e R­g n ilc y c e Rla itn e to p
A1 A2 A3 A4 A5 B1 B2 B3 B4 B5 B6 B7 C1 C2 C3 C4 D
X X X MND MND MND MND MNR MNR MNR MND MND X X X X X
RESULTS OF THE LCA - ENVIRONMENTAL IMPACT according to EN 15804+A2: 1 tonne CHQ-, bearing-, spring steel –
automotive wire
Parameter Unit A1-A3 C1 C2 C3 C4 D
Global Warming Potential total (GWP­total) kg CO 2 eq 2.93E+03 0 3.02E+00 0 2.42E+00 ­1.45E+03
Global Warming Potential fossil fuels (GWP­fossil) kg CO 2 eq 2.9E+03 0 3E+00 0 2.44E+00 ­1.45E+03
Global Warming Potential biogenic (GWP­biogenic) kg CO 2 eq 2.09E+01 0 ­3.56E­03 0 ­2.5E­02 ­9.41E­01
Global Warming Potential luluc (GWP­luluc) kg CO 2 eq 1E+00 0 2.44E­02 0 2.44E­03 2.1E­01
Depletion potential of the stratospheric ozone layer (ODP) kg CFC11 eq 8.57E­12 0 5.9E­16 0 5.77E­15 ­2.42E­12
Acidification potential of land and water (AP) mol H+ eq 8.99E+00 0 9.92E­03 0 7.78E­03 ­2.61E+00
Eutrophication potential aquatic freshwater (EP­freshwater) kg P eq 1.62E­02 0 8.88E­06 0 1.86E­06 ­2.97E­04
Eutrophication potential aquatic marine (EP­marine) kg N eq 2.17E+00 0 4.55E­03 0 1.93E­03 ­3.88E­01
Eutrophication potential terrestrial (EP­terrestrial) mol N eq 2.31E+01 0 5.08E­02 0 2.12E­02 ­3.79E+00
Formation potential of tropospheric ozone photochemical oxidants kg NMVOC
7.24E+00 0 8.94E­03 0 6.08E­03 ­1.99E+00
(POCP) eq
Abiotic depletion potential for non fossil resources (ADPE) kg Sb eq 4.5E­03 0 2.65E­07 0 1.68E­07 ­3.16E­03
Abiotic depletion potential for fossil resources (ADPF) MJ 2.68E+04 0 3.98E+01 0 3.56E+01 ­1.26E+04
m3 world eq
Water use (WDP) 5.01E+02 0 2.77E­02 0 ­2.89E­02 ­2.85E+02
deprived
RESULTS OF THE LCA - INDICATORS TO DESCRIBE RESOURCE USE according to EN 15804+A2: 1 tonne CHQ-, bearing-,
spring steel – automotive wire
Parameter Unit A1-A3 C1 C2 C3 C4 D
Renewable primary energy as energy carrier (PERE) MJ 2.15E+03 0 2.29E+00 0 2.57E+00 1.16E+03
Renewable primary energy resources as material utilization
MJ 1.39E+02 0 0 0 0 0
(PERM)
Total use of renewable primary energy resources (PERT) MJ 2.29E+03 0 2.29E+00 0 2.57E+00 1.16E+03
Non renewable primary energy as energy carrier (PENRE) MJ 2.68E+04 0 4E+01 0 3.56E+01 ­1.26E+04
Non renewable primary energy as material utilization (PENRM) MJ 5.68E+00 0 0 0 0 0
Total use of non renewable primary energy resources (PENRT) MJ 2.69E+04 0 4E+01 0 3.56E+01 ­1.26E+04
Use of secondary material (SM) kg 1.16E+02 0 0 0 0 8.56E+02
Use of renewable secondary fuels (RSF) MJ 0 0 0 0 0 0
Use of non renewable secondary fuels (NRSF) MJ 0 0 0 0 0 0
Use of net fresh water (FW) m3 1.5E+01 0 2.62E­03 0 3.67E­04 ­6.4E+00
RESULTS OF THE LCA – WASTE CATEGORIES AND OUTPUT FLOWS according to EN 15804+A2:
1 tonne CHQ-, bearing-, spring steel – automotive wire
Parameter Unit A1-A3 C1 C2 C3 C4 D
Hazardous waste disposed (HWD) kg 7.92E­06 0 2.11E­09 0 6.3E­09 3.53E­06
Non hazardous waste disposed (NHWD) kg 7.07E+01 0 6.27E­03 0 5.01E+01 1.52E+02
Radioactive waste disposed (RWD) kg 1.35E­01 0 7.25E­05 0 4.05E­04 4.58E­04
Components for re­use (CRU) kg 0 0 0 0 0 0
Materials for recycling (MFR) kg 0 0 0 9.5E+02 0 0
Materials for energy recovery (MER) kg 0 0 0 0 0 0
Exported electrical energy (EEE) MJ 0 0 0 0 0 0
Exported thermal energy (EET) MJ 0 0 0 0 0 0
RESULTS OF THE LCA – additional impact categories according to EN 15804+A2-optional:
1 tonne CHQ-, bearing-, spring steel – automotive wire
Parameter Unit A1-A3 C1 C2 C3 C4 D
Disease
Incidence of disease due to PM emissions (PM) ND ND ND ND ND ND
incidence
Human exposure efficiency relative to U235 (IR) kBq U235 eq ND ND ND ND ND ND
7 Environmental Product Declaration ­ voestalpine Wire Austria GmbH ­ Drawn Wire – Cold Heading Wire
Comparative toxic unit for ecosystems (ETP­fw) CTUe ND ND ND ND ND ND
Comparative toxic unit for humans (carcinogenic) (HTP­c) CTUh ND ND ND ND ND ND
Comparative toxic unit for humans (noncarcinogenic) (HTP­nc) CTUh ND ND ND ND ND ND
Soil quality index (SQP) SQP ND ND ND ND ND ND
The additional and optional impact categories according to EN 15804+A2 are not declared, as the uncertainty of these indicators is to
be classified as high.
Disclaimer 1 – for the indicator potential human exposure efficiency relative to U235:
This impact category deals mainly with the eventual impact of low dose ionizing radiation on human health of the nuclear fuel cycle. It
does not consider effects due to possible nuclear accidents, occupational exposure nor radioactive waste disposal in underground
facilities. Potential ionizing radiation from the soil, from radon and from some construction materials is also not measured by this
indicator.
Disclaimer 2 – for the indicators abiotic depletion potential for non­fossil resources, abiotic depletion potential for fossil resources, water
(user) deprivation potential, deprivation weighted water consumption, eutrophication fraction of nutrients reaching freshwater end
compartment, potential comparative toxic unit for humans cancerogenic, potential comparative toxic unit for humans not cancerogenic,
potential soil quality index:
The results of this environmental impact indicator shall be used with care as the uncertainties on these results are high or as there is
limited experience with the indicator.
6. LCA: Interpretation
The following interpretation contains a summary of the LCA bearing­, spring steel – automotive wire.
results referenced to a declared unit of 1 tonne of CHQ­,
A comparison of the individual lifecycle phases results in a clear Most of the potential environmental impacts of the production
dominance of the production phase (modules A1–A3). The phase (module A1–A3) of the CHQ­, bearing­, spring steel –
environmental effects in the production phase are mainly automotive wire can be traced back to the upstream supply of
dominated by the direct process emissions of billet production. the wire rod. The production of automotive wire at the
As a result of product recyclability, the material removed at the production site at Bruck contributes app. 5 % to global warming
end of life can substitute primary steel. According to the set potential.
method, the first step is to saturate the secondary material used
in module A with material from module C. The excess amount A linear correlation of the environmental impacts with the
from module C ('net flow') can substitute primary steel and product weight is to be expected. Therefore, the conversion
leads to corresponding substitution potentials in module D. from the declared unit to a specific product is possible using a
The environmental impact of the transport of the products to mass­specific scaling factor.
recycling (C2) as well as landfilling of the losses at the end of
life (C4) represents a minor contribution to the overall All primary data were specifically broken down to the declared
environmental impact of the product. product group. As a result, the representativity of the results for
the declared product group is to be expected as high.
8 Environmental Product Declaration ­ voestalpine Wire Austria GmbH ­ Drawn Wire – Cold Heading Wire
7. Requisite evidence
Not relevant for this EPD.
8. References
Standards Article 59 (10) of the REACH Regulation Helsinki: European
Chemicals Agency.
EN 10027-2
DIN EN 10027­2:2015­07, Designation systems for steels ­ Part EMAS III
2: Numerical system. Regulation (EC) No 1221/2009 of the European parliament and
of the council of 25 November 2009 on the voluntary
EN 10089 participation by organisations in a Community eco­management
DIN EN 10089­2:2003­04, Hot rolled steels for quenched and and audit scheme (EMAS), repealing Regulation (EC) No
tempered springs ­ Technical delivery conditions. 761/2001 and Commission Decisions 2001/681/EC and
2006/193/EC.
EN 10263
DIN EN 10263­1:2018­02, Steel rod, bars and wire for cold European Waste Catalogue
heading and cold extrusion ­ Part 1: General technical delivery Guidance on classification of waste according to EWC Stat
conditions. categories. Supplement to the Manual for the Implementation of
the Regulation (EC) No 2150/2002 on Waste Statistics.
EN 10278 Commission of the European Communities, EUROSTAT.
DIN EN 10278:1999­12, Dimensions and tolerances of bright
steel products. GaBi
GaBi 10, Software System and Database for Life Cycle
EN 15804 Engineering. DB 2021.1. Sphera, 1992­2021. Available in:
DIN EN 15804:2012+A2:2019+AC:2021, Sustainability of http://documentation.gabisoftware.com
construction works — Environmental Product Declarations —
Core rules for the product category of construction products. IBU 2021
Institut Bauen und Umwelt e.V.: General guidance for the EPD
ISO 683-17 program of the Institut Bauen und Umwelt e.V.. (IBU). Version
DIN EN ISO 683­17:2015­02, Heat­treated steels, alloy steels 2.0, Berlin: Institut Bauen und Umwelt e.V., 2021.
and free­cutting steels ­ Part 17: Ball and roller bearing steels. www.ibu­epd.com
ISO 9001 Key to Steel
ISO 9001:2015, Quality management systems – Requirements. Key to Steel (Stahlschlüssel) 2019, 25. edition, 2023, Verlag
Stahlschlüssel Wegst GmbH, Germany.
ISO 10270-1
DIN EN ISO 10270­1:2011, Steel wire for mechanical springs ­ ökobaudat 2022
Part 1: Patented cold drawn unalloyed spring steel wire. ökobaudat 2022. EN 15804 and BNB compliant data for over
700 building products.
ISO 14001
ISO 14001:2015, Environmental management systems – Ordinance on Biocide Products
Requirements with guidance for use. Regulation (EU) No 528/2012 of the European Parliament and
of the Council of 22 May 2012 concerning the making available
ISO 14025 on the market and use of biocidal products.
DIN EN ISO 14025:2011­10, Environmental labels and
declarations ­ Type III environmental declarations ­ Principles PCR Part A
and procedures. Product category rules for building­related products and
services. Part A: Calculation rules for life cycle assessment and
ISO 14044 project report requirements according to EN 15804+A2:2019.
DIN EN ISO 14044:2006­10, Environmental management ­ Life Version 1.3. Berlin: Institut Bauen und Umwelt e.V.. (ed.), 2022.
cycle assessment ­ Requirements and guidance.
PCR: Structural steels
ISO 45001 Product category rules for building­related products and
DIN EN ISO 45001:2018­03, Occupational health and safety services. Part B: Requirements for the EPD for structural steels.
management systems ­ Requirements with guidance for use. Version v0. Berlin: Institut Bauen und Umwelt e.V., 08.03.2023.
ISO 50001 worldsteel 2014
ISO 50001:2018, Energy Management Systems. World Steel Association, February 14, 2014: A methodology to
determine the LCI of steel industry co­products.
Further references
worldsteel 2019
Candidate list World Steel Association, 2019: Life cycle inventory
Candidate List of Substances of Very High Concern (ECHA methodology report.
Candidate List) of 16.01.2020, published in accordance with
9 Environmental Product Declaration ­ voestalpine Wire Austria GmbH ­ Drawn Wire – Cold Heading Wire
Publisher
Institut Bauen und Umwelt e.V. +49 (0)30 3087748­ 0
Hegelplatz 1 info@ibu­epd.com
10117 Berlin www.ibu­epd.com
Germany
Programme holder
Institut Bauen und Umwelt e.V. +49 (0)30 3087748­ 0
Hegelplatz 1 info@ibu­epd.com
10117 Berlin www.ibu­epd.com
Germany
Author of the Life Cycle Assessment
Daxner & Merl GmbH +43 676 849477826
Schleifmühlgasse 13/24 office@daxner­merl.com
1040 Wien www.daxner­merl.com
Austria
Owner of the Declaration
voestalpine AG +43/50304/15­0
voestalpine­Straße 3 info@voestalpine.com
4020 Linz www.voestalpine.com
Austria
10 Environmental Product Declaration ­ voestalpine Wire Austria GmbH ­ Drawn Wire – Cold Heading Wire
