ENVIRONMENTAL PRODUCT DECLARATION
as per ISO 14025 and EN 15804+A2
Owner of the Declaration Ideal Standard International NV
Publisher Institut Bauen und Umwelt e.V. (IBU)
Programme holder Institut Bauen und Umwelt e.V. (IBU)
Declaration number EPD-IDE-20230005-IBD1-EN
Issue date 24.05.2023
Valid to 23.05.2028
Ceramic Vitreous China product
Ideal Standard International
www.ibu-epd.com | https://epd-online.com
1. General Information
Ideal Standard International Ceramic Vitreous China product
Programme holder Owner of the declaration
IBU – Institut Bauen und Umwelt e.V. Ideal Standard International NV
Hegelplatz 1 Da Vincilaan 2
10117 Berlin 1935 Zaventem
Germany Belgium
Declaration number Declared product / declared unit
EPD-IDE-20230005-IBD1-EN 1 kg of ceramic vitreous china product
This declaration is based on the product category rules: Scope:
Sanitary ceramics, 01.08.2021 The EPD contains the result of 1 kg of ceramic vitreous china product
(PCR checked and approved by the SVR) produced by Ideal Standard. It is representative for those ceramic products
categories: bowls (mounted and floor standing), urinals, bidets,
washbasins and pedestals, manufactured in Sevlievo (Bulgaria), Armitage
Issue date (United Kingdom) and Teplice (Czech Republique). As the result is for 1kg
of ceramic, the user can easily calculate the results for ceramic products,
24.05.2023
noted above according to the weight. The factory in Egypt is not included
in the scope of the EPD.
Valid to
Foreground data has been provided directly by Ideal Standard and
23.05.2028 background LCA data is based on Ecoinvent 3.8 and Industry 2.0 data.
The owner of the declaration shall be liable for the underlying information
and evidence; the IBU shall not be liable with respect to manufacturer
information, life cycle assessment data and evidences.
The EPD was created according to the specifications of EN 15804+A2. In
the following, the standard will be simplified as EN 15804.
Verification
The standard EN 15804 serves as the core PCR
Independent verification of the declaration and data according to ISO
14025:2011
Dipl.-Ing. Hans Peters
(Chairman of Institut Bauen und Umwelt e.V.) internally X externally
Florian Pronold Vito D'Incognito,
(Managing Director Institut Bauen und Umwelt e.V.) (Independent verifier)
1 Environmental Product Declaration - Ideal Standard International - Ceramic Vitreous China product
2. Product
· 20-30 % clay
2.1 Product description/Product definition · 20-30 % China clay
This product under study is 1 kg of standard white vitreous · 20-30 % Feldspar
china product. Product categories included in this EPD are: · 20-30 % Silica
bowls (mounted and floor standing), urinals, bidets, washbasins · <5 % Glaze
and pedestals, (manufacturing sites are listed above).
This product/article/at least one partial article contains
The manufacturer can - within the framework of the European substances listed in the candidate list (date: 16.05.2023)
Regulation N° 305/2011 (CPR) - present the Declaration of exceeding 0.1 percentage by mass: no
Performance (DOP) of the product confirming that the product
has a CE marking. This product/article/at least one partial article contains other
carcinogenic, mutagenic, reprotoxic (CMR) substances in
2.2 Application
categories 1A or 1B which are not on the candidate list,
The products are used in private and public bathrooms. The exceeding 0.1 percentage by mass: no
product can be used in new construction and renovation work
for hygienic and household use. Biocide products were added to this construction product or it
has been treated with biocide products (this then concerns a
2.3 Technical Data
treated product as defined by the (EU) Ordinance on Biocide
Constructional data Products No. 528/2012): no
Name Value Unit 2.6 Manufacture
Minimum 1
Crazing test Internal test - 1hr in autoclave 1. Slip preparation
cycle without -
with 5bar steam Production of the ceramic mixture (slip) and
crazing
unloading/storage of raw materials in the area.
Water absorption EN997 for WC pans 2. Glaze preparation
(toilets) and so by extension to the <0.5 % Production of glaze with needed colour.
Vitreous China products 3. Casting shop
Minimum 1 Casting of ceramic products in different moulds.
Impact resistance Internal test – Ball
drop without - 4. Dryers
bearing dropped from fixed height
breaking Drying is the process of taking off the humidity and the
Resistance to temperature change EN final results are dried products.
14688 for Wash Basins. 1000 hot (75 No visible 5. White inspection
-
degC) / cold (15 degC) water cycles damage The first inspection of dried ceramic products. The main
without visible damage focus is checking the quality and cleaning the surface of
Resistance to chemicals and staining EN the products. At the end of the process the products are
14688 for Wash Basins therefore by grouped in three different directions: A grade products,
extension to other Ceramic Products. No remaining products for repairing and scrap.
Specific chemicals in contact then cleaned chemical - 6. Spraying
with specific apparatus without permanent evident Covering the ceramic product with glaze
marking 7. Kilns
Firing of ceramic products
Resistance to abrasion EN 14688 for
8. Gloss inspection
Wash Basins therefore by extension to No scratches
Final inspection for visual control of all products for
other Ceramic Products. Loaded diamond through outer -
visible defects. Separating the products again in three
tool (scratch) / Loaded abrasive paper (glaze) layer
groups: for packaging, for repairing by hand or for
wheel (abrasion) for repeated cycles.
grinding machines and scrap (pitcher).
Load resistance 400 Kg
9. Packaging
The manufacturer can - within the framework of the European Different kinds of activities for the packaging of the
Regulation N° 305/2011 (CPR) - present the Declaration of products.
Performance (DOP) of the product confirming that the product
has a CE marking. *Moulds making Development of a new matrix for
production of gypsum moulds for casting and repairing
2.4 Delivery status of the damaged matrix.
The products are packed: wooden pallet, PE plastic and
cardboard, and are accompanied with an instruction and *Mould shop Production of gypsum moulds for casting
guarantee sheet. ceramic products and polyurethane setters for
supporting the casting process.
The products can come in different shapes and dimensions. An
overview of all included products in this EPD can be provided 2.7 Environment and health during manufacturing
by Ideal Standard. Environmental, occupational health, safety and quality
management at the Ideal Standard plants are in accordance
2.5 Base materials/Ancillary materials with the following standards:
This EPD include different product categories: bowls, urinals,
• ISO 14001
bidets, washbasin and pedestals.
• ISO 9001
• ISO 45001
The composition of the Vitreous china ceramic is:
2 Environmental Product Declaration - Ideal Standard International - Ceramic Vitreous China product
2.8 Product processing/Installation 2.13 Extraordinary effects
It is considered that there is no assembly waste, based on the Fire
fact that the product is prefabricated and installed by hand. Not subjected to fire classification
Water
2.9 Packaging No risks are expected to occur in terms of environmental and
A wooden pallet, PE plastic bag and cardboard are used to human health.
pack and transport the product to the supplier/customer. The
product is also accompanied by an instruction and guarantee Mechanical destruction
sheet. In case of mechanical destruction, no risks are expected to
occur in terms of environment and human health.
2.10 Condition of use
The product will not change in material composition over the 2.14 Re-use phase
reference service life. It is possible to recycle ceramic products in the production
process. This is already applied for production waste. The
2.11 Environment and health during use
recycling of post-consumer waste depends on the sorting and
Under normal conditions of use, the product do not cause any take-back of these waste streams at the demolition site.
adverse health effects or release of volatile organic compounds
(VOCs) into indoor air. 2.15 Disposal
According to the average European end-of-life scenario
No environmental impact on water, air or soil is expected. described in Annexe C of the Product Environmental Footprint
Pilots (PEFCR) 6.3 guidance, the following disposal scenarios
2.12 Reference service life
have been considered: 100 % of the ceramic is landfilled.
The reference service life is not relevant, as module B is not
considered. 2.16 Further information
Description of the influences on the ageing of the product when Additional information on vitreous china ceramic products
applied in accordance with the rules of technology. manufactured by Ideal Standard can be found on:
https://www.idealstandard.com/
3. LCA: Calculation rules
No further approximations have been made to replace the
3.1 Declared Unit missing data, as they were considered to be not relevant based
The calculation made in the tool is relevant to 1 kg of ceramic on the first iterations of the results.
vitreous china products.
3.4 Cut-off criteria
The average weighted product is manufactured in Bulgaria.
• Big bags used as packaging of some raw materials for
Then, this EPD is calculated using the production data of the
the ceramic production, as they are reused.
factory in Bulgaria.
• For production waste only most relevant production
waste streams have been considered (waste of ancillary
However, a variability study has been performed to show that
materials and smaller waste flows have been excluded).
the production in Bulgaria is representative for the production
• Only most relevant ancillary materials have been
by Ideal Standard in the United Kingdom and the Czech
selected based on consumption rate and importance in
Republique. The difference over the total life cycle of the
the production process.
product is less than 40 % for the three most relevant impact
• Environmental impacts caused by the personnel of the
indicators (based on PEF single score), respectively Global
production plants are not included in the LCA, e.g.
warming potential, Resource use fossils and Particulate matter.
waste from the cafeteria and sanitary installations or
environmental effects caused by commuter traffic.
Name Value Unit Cooling of the plants in order to ensure a comfortable
Declared unit 0.001 t indoor climate for the personnel for example is also
neglected.
The user can easily calculate the results for ceramic products,
noted above according to the weight. The products typically
3.5 Background data
weigh between 4.5 and 38.8 kg.
Ecoinvent 3.8 and Industry 2.0
3.6 Data quality
Foreground data is specific to Ideal Standard and is collected
3.2 System boundary
for the reference year 2021. Background data is based on
Cradle-to-gate with options, including modules A4, A5, C1, C2,
Ecoinvent 3.8 which is released in September 2021.
C3, C4 and D
3.3 Estimates and assumptions The LCA background report includes a variability study
between the different factory plants, respectively Sevlievo
The following processes are excluded because data was not
(Bulgaria), Armitage (United Kingdom) and Teplice (Czech
available:
Republique). The results show that over the total life cycle (A1-
• Packaging of raw materials used to produce the glaze of C4) the variance is less than 40 %.
the ceramic products,
• Transport of the packaging of the final product, 3.7 Period under review
• Packaging and transport of ancillary materials used The data collected by Ideal Standard is based on data from the
during the production process, production year 2021.
• Packaging and transport of ancillary materials used
during installation, 3.8 Geographic Representativeness
3 Environmental Product Declaration - Ideal Standard International - Ceramic Vitreous China product
Land or region, in which the declared product system is consumption, production waste, ancillary materials and
manufactured, used or handled at the end of the product´s emissions are based on factory averages (total amount
lifespan: Europe in the factory converted to 1 kg based on the total
production volume in kg).
3.9 Allocation 3.10 Comparability
Basically, a comparison or an evaluation of EPD data is only
• Amounts of the raw materials/components (modules A1
possible if all the data sets to be compared were created
and A2) and the packaging of the final product have
according to EN 15804 and the building context, respectively
been extracted from recipe used in the respective
the product-specific characteristics of performance, are taken
factory. No allocation was necessary. Note that the
into account. Used background databases: Ecoinvent 3.8 and
production losses have been added to the recipe.
Industry 2.0
• The data for the production process (module A3) i.e
input and outputs such as energy consumption, water
4. LCA: Scenarios and additional technical information
End of life (C1-C4)
Characteristic product properties of biogenic carbon
According to the average European end-of-life scenario
The product does not contain biogenic carbon, but its
described in Annexe C of the Product Environmental Footprint
accompanying packaging contains 8.77E-02 kg C per product
Pilots (PEFCR) 6.3 guidance, the following disposal scenarios
in the form of paper, cardboard and wooden pallets.
have been considered: 100 % of the ceramic parts are
Information on describing the biogenic Carbon Content at landfilled.
factury gate
Name Value Unit
Name Value Unit
Collected as mixed construction waste 1 kg
kg
Biogenic carbon content in product - Landfille of ceramic 1 Kg
C
Biogenic carbon content in accompanying kg Reuse, recovery and/or recycling potentials (D), relevant
0.0877
packaging C scenario information
Module D contains low benefits and loads of recycling of the
packaging of the final product and the benefits of energy
recovery during the incineration of the plastic. There is no
Transport to the building site (A4)
benefits and loads from the end of life of the product, because
Name Value Unit the product is 100 % landfilled.
Litres of fuel 260 l/100km Name Value Unit
Transport distance 2000 km
Capacity utilisation (including empty runs) - %
Gross density of products transported - kg/m3
Capacity utilisation volume factor - -
Installation into the building (A5)
It is considered that there is no assembly waste, based on the
fact that the product is prefabricated and installed by hand.
Only the impact of packaging waste has been considered.
Name Value Unit
Packaging waste (paper and cardboard) PEF
EOL scenario Europe for coverage carton
0,085 Kg
packaging: 11 % incineration; 75 % recycling;
14 % landfill
Packaging waste (PE) PEF EOL scenario
Europe for PE packaging: 32 % incineration; 29 0,039338 Kg
% recycling; 39 % landfill
Packaging waste (wooden pallet) PEF EOL
scenario Europe for wooden pallets: 32 % 0,110 Kg
incineration; 30 % recycling; 38 % landfill
4 Environmental Product Declaration - Ideal Standard International - Ceramic Vitreous China product
5. LCA: Results
DESCRIPTION OF THE SYSTEM BOUNDARY (X = INCLUDED IN LCA; ND = MODULE OR INDICATOR NOT DECLARED; MNR =
MODULE NOT RELEVANT)
Benefits and
Construction loads beyond
Product stage Use stage End of life stage
process stage the system
boundaries
la ire ta m w a Ry lp p u s tro p s n a rT g n iru tc a fu n a M e h t m o rf tro p s n a rTe tis e h t o t e ta g y lb m e s s A e s U e c n a n e tn ia M ria p e R tn e m e c a lp e R tn e m h s ib ru fe R y g re n e la n o ita re p Oe s u re ta w la n o ita re p Oe s u n o itc u rts n o c -e Dn o itilo m e d tro p s n a rT g n is s e c o rp e ts a W la s o p s iD -e s u e R-y re v o c e R-g n ilc y c e Rla itn e to p
A1 A2 A3 A4 A5 B1 B2 B3 B4 B5 B6 B7 C1 C2 C3 C4 D
X X X X X MND MND MNR MNR MNR MND MND X X X X X
RESULTS OF THE LCA - ENVIRONMENTAL IMPACT according to EN 15804+A2: 1 Kg Declared unit
Parameter Unit A1 A2 A3 A4 A5 C1 C2 C3 C4 D
GWP-total kg CO 2 eq 7.5E-02 1.45E-01 1.25E+00 4.03E-01 3.5E-01 1.54E-04 8.15E-03 0 6.53E-03 -2.11E-01
GWP-fossil kg CO 2 eq 7.47E-02 1.45E-01 1.54E+00 4.03E-01 4.72E-02 1.52E-04 8.14E-03 0 6.5E-03 -6.24E-02
GWP-
biogenic kg CO 2 eq 1.9E-04 5.03E-05 -2.94E-01 1.44E-04 3.02E-01 8.44E-07 2.91E-06 0 2.92E-05 -1.48E-01
GWP-luluc kg CO 2 eq 8.02E-05 6.2E-05 8.9E-04 1.61E-04 3.16E-06 3.6E-07 3.26E-06 0 3.61E-06 -1.46E-04
ODP kg CFC11 eq 1.09E-08 3.32E-08 1.56E-07 9.33E-08 1.67E-09 7.66E-12 1.89E-09 0 2.22E-09 -5.92E-09
AP mol H+ eq 4.35E-04 7.78E-04 5.19E-03 1.14E-03 4.23E-05 8.65E-07 2.31E-05 0 5E-05 -2.79E-04
EP-
kg P eq 3.58E-06 9.9E-07 1.23E-04 2.87E-06 1.07E-07 1.63E-08 5.81E-08 0 3.29E-07 -2.99E-06
freshwater
EP-marine kg N eq 7.24E-05 1.74E-04 8.92E-04 2.27E-04 1.63E-05 1.1E-07 4.6E-06 0 1.8E-05 -6.89E-05
EP-terrestrial mol N eq 8.24E-04 1.93E-03 8.91E-03 2.53E-03 1.66E-04 1.27E-06 5.12E-05 0 2E-04 -7.56E-04
kg NMVOC
POCP 2.34E-04 6.05E-04 2.62E-03 9.73E-04 4.97E-05 3.5E-07 1.97E-05 0 5.66E-05 -2.55E-04
eq
ADPE kg Sb eq 3.8E-07 3.72E-07 1.31E-06 1.09E-06 2.04E-08 8.23E-10 2.21E-08 0 1.67E-08 -2.16E-07
ADPF MJ 1.22E+00 2.17E+00 2.86E+01 6.1E+00 1.12E-01 3.23E-03 1.23E-01 0 1.68E-01 -1.46E+00
m3 world eq
WDP 9.59E-02 6.39E-03 4.95E-01 1.86E-02 6.35E-04 3.78E-05 3.76E-04 0 5.69E-04 -7.08E-02
deprived
GWP = Global warming potential; ODP = Depletion potential of the stratospheric ozone layer; AP = Acidification potential of land and water; EP =
Eutrophication potential; POCP = Formation potential of tropospheric ozone photochemical oxidants; ADPE = Abiotic depletion potential for non-fossil
resources; ADPF = Abiotic depletion potential for fossil resources; WDP = Water (user) deprivation potential)
RESULTS OF THE LCA - INDICATORS TO DESCRIBE RESOURCE USE according to EN 15804+A2: 1 Kg Declared unit
Parameter Unit A1 A2 A3 A4 A5 C1 C2 C3 C4 D
PERE MJ 1.27E-01 2.93E-02 1.29E+00 8.58E-02 6.53E-01 6.41E-04 1.74E-03 0 8.86E-03 0
PERM MJ 0 0 2.92E+00 0 -2.14E+00 0 0 0 0 1.49E+00
PERT MJ 1.3E-01 3E-02 4.21E+00 9E-02 -1.49E+00 0 0 0 1E-02 1.49E+00
PENRE MJ 1.42E+00 2.17E+00 3.14E+01 6.13E+00 6.5E-01 3.83E-03 1.24E-01 0 1.76E-01 0
PENRM MJ 0 0 1.67E-01 0 -1.02E+00 0 0 0 0 4.85E-01
PENRT MJ 1.43E+00 2.18E+00 3.3E+01 6.14E+00 -3.7E-01 3.8E-03 1.24E-01 0 1.76E-01 4.85E-01
SM kg 0 0 0 0 0 0 0 0 0 1.09E-01
RSF MJ 0 0 0 0 0 0 0 0 0 0
NRSF MJ 0 0 0 0 0 0 0 0 0 0
FW m3 1.6E-03 1.53E-04 7.05E-03 4.49E-04 5.5E-05 2.43E-06 9.08E-06 0 1.71E-04 -1.63E-03
PERE = Use of renewable primary energy excluding renewable primary energy resources used as raw materials; PERM = Use of renewable primary
energy resources used as raw materials; PERT = Total use of renewable primary energy resources; PENRE = Use of non-renewable primary energy
excluding non-renewable primary energy resources used as raw materials; PENRM = Use of non-renewable primary energy resources used as raw
materials; PENRT = Total use of non-renewable primary energy resources; SM = Use of secondary material; RSF = Use of renewable secondary fuels;
NRSF = Use of non-renewable secondary fuels; FW = Use of net fresh water
RESULTS OF THE LCA – WASTE CATEGORIES AND OUTPUT FLOWS according to EN 15804+A2:
1 Kg Declared unit
Parameter Unit A1 A2 A3 A4 A5 C1 C2 C3 C4 D
HWD kg 1.49E-06 5.4E-06 2.66E-05 1.59E-05 2.75E-07 2.45E-09 3.22E-07 0 2.08E-07 -1.09E-06
NHWD kg 5.77E-02 1.06E-01 5.17E-01 3.2E-01 7.53E-02 1.18E-05 6.47E-03 0 1E+00 -7.94E-03
RWD kg 5.36E-06 1.47E-05 7.71E-05 4.13E-05 7.14E-07 2.36E-08 8.34E-07 0 1.07E-06 -3.51E-06
CRU kg 0 0 0 0 0 0 0 0 0 0
MFR kg 0 0 0 0 1.09E-01 0 0 0 0 -1.09E-01
MER kg 0 0 0 0 0 0 0 0 0 0
EEE MJ 0 0 0 0 1.19E-01 0 0 0 0 -1.19E-01
EET MJ 0 0 0 0 2.37E-01 0 0 0 0 -2.37E-01
5 Environmental Product Declaration - Ideal Standard International - Ceramic Vitreous China product
HWD = Hazardous waste disposed; NHWD = Non-hazardous waste disposed; RWD = Radioactive waste disposed; CRU = Components for re-use;
MFR = Materials for recycling; MER = Materials for energy recovery; EEE = Exported electrical energy; EET = Exported thermal energy
RESULTS OF THE LCA – additional impact categories according to EN 15804+A2-optional:
1 Kg Declared unit
Parameter Unit A1 A2 A3 A4 A5 C1 C2 C3 C4 D
Disease
PM 3.78E-09 1.1E-08 3.67E-08 3.24E-08 7.55E-10 2.39E-12 6.54E-10 0 1.03E-09 -5.51E-09
incidence
IR kBq U235 eq 5.84E-03 9.41E-03 9.07E-02 2.65E-02 4.73E-04 2.86E-05 5.36E-04 0 6.95E-04 -3.66E-03
ETP-fw CTUe 1.29E+00 1.68E+00 6.43E+00 4.79E+00 1.23E-01 2.04E-03 9.69E-02 0 1E-01 -6.35E-01
HTP-c CTUh 3.68E-11 5.82E-11 5.34E-10 1.54E-10 2.12E-11 6.27E-14 3.12E-12 0 2.89E-12 -2.56E-11
HTP-nc CTUh 1E-09 1.66E-09 1.18E-08 4.84E-09 1.7E-10 2E-12 9.79E-11 0 6.06E-11 -5.73E-10
SQP SQP 1.17E+00 1.42E+00 2.07E+01 4.26E+00 1.02E-01 5.85E-04 8.6E-02 0 3.27E-01 -1.56E+01
PM = Potential incidence of disease due to PM emissions; IR = Potential Human exposure efficiency relative to U235; ETP-fw = Potential comparative
Toxic Unit for ecosystems; HTP-c = Potential comparative Toxic Unit for humans (cancerogenic); HTP-nc = Potential comparative Toxic Unit for humans
(not cancerogenic); SQP = Potential soil quality index
Disclaimer 1 – for the indicator “Potential Human exposure efficiency relative to U235”. This impact category deals mainly with the
eventual impact of low-dose ionizing radiation on human health of the nuclear fuel cycle. It does not consider effects due to possible
nuclear accidents, occupational exposure or radioactive waste disposal in underground facilities. Potential ionizing radiation from the
soil, radon and from some construction materials is also not measured by this indicator.
Disclaimer 2 – for the indicators “abiotic depletion potential for non-fossil resources”, “abiotic depletion potential for fossil resources”,
“water (user) deprivation potential, deprivation-weighted water consumption”, “potential comparative toxic unit for ecosystems”,
“potential comparative toxic unit for humans – cancerogenic”, “Potential comparative toxic unit for humans - not cancerogenic”,
“potential soil quality index”. The results of this environmental impact indicator shall be used with care as the uncertainties on these
results are high as there is limited experience with the indicator.
6. LCA: Interpretation
The manufacturing process (module A3), in particular the weight of the products. The impact of the raw materials is less
energy consumption, has the largest contribution on all impact significant. There is no benefits and loads from the end of life of
categories. Besides the manufacturing, also the transport to the the product, because the product is 100 % landfilled.
installation site (A4) has a significant contribution, due to the
7. Requisite evidence
8. References
Standards
ISO 14044
EN 997 ISO 14044:2006: Environmental management – Life cycle
WC pans and WC suites with integral trap - constructional and assessment – Requirements and guidelines.
performance requirements.
ISO 45001
EN 14688 ISO 45001:2018: Occupational health and safety management
Sanitary appliances. Wash basins. Functional requirements and systems Requirements with guidance for use
test methods
PCR Part A
EN15804 Calculation rules for the Life Cycle Assessment and
EN 15804:2012+A2:2019+AC:2021, Sustainability of Requirements on the Background Report, Institut Bauen und
construction works — Environmental Product Declarations — Umwelt e.V., www.bauumwelt.com.
Core rules for the product category of construction products.
PCR Part B
ISO 9001 Institut Bauen und Umwelt e.V, Berlin (pub.): PCR Guidance-
ISO 9001:2015: Quality management systems — Requirements Texts for Building-Related Products and Services From the
range of Environmental Product Declarations of Institute
ISO 14001 Construction and Environment e.V. (IBU) : Requirements on the
ISO 14001:2015: Environmental management systems — EPD for Toilet set
Requirements with guidance for use
Further references
ISO 14025
EN ISO 14025:2011, Environmental labels and declarations — Biocide Products No. 528/2012
Type III environmental declarations — Principles and Biocide Products No. 528/2012 EU, REGULATION (EU) No
procedures. 528/2012 OF THE EUROPEANPARLIAMENT
ISO 14040 CPR
ISO 14040:2006: Environmental management – Life cycle European Regulation N° 305/2011 (CPR)
assessment – Principles and framework
6 Environmental Product Declaration - Ideal Standard International - Ceramic Vitreous China product
Ecoinvent Industry 2.0 (from PlasticsEurope, worldsteel and ERASM) LCA
Wernet, G., Bauer, C., Steubing, B., Reinhard, J., Moreno-Ruiz, database as integrated in SimaPro 9.3.0.3.
E., and Weidema, B., 2016. The ecoinvent database version 3
(part I): overview and methodology. The International Journal of PEFCR
Life Cycle Assessment, [online] 21(9), pp.1218–1230. Available European commission (2018). Product Environmental Footprint
at:http://link.springer.com/10.1007/s11367-016-1087-8 Category Rules PEFCR Guidance, version 6.3.
IBU Pré Consultants (2021)
IBU 2021. Institut Bauen und Umwelt e.V.: General Instructions SimaPro 9.3.0.3 [Computer Software]. Amersfoort, The
for the EPD programme of Institut Bauen und Umwelt e.V., Netherlands.
Version 2.0, Berlin: Institut Bauen und Umwelt e.V., 2021
www.ibu-epd.com REACH candidate list
ECHA, REACH Candidate List of substances of very
Industry 2.0 highconcern for Authorisation
7 Environmental Product Declaration - Ideal Standard International - Ceramic Vitreous China product
Publisher
Institut Bauen und Umwelt e.V. +49 (0)30 3087748- 0
Hegelplatz 1 info@ibu-epd.com
10117 Berlin www.ibu-epd.com
Germany
Programme holder
Institut Bauen und Umwelt e.V. +49 (0)30 3087748- 0
Hegelplatz 1 info@ibu-epd.com
10117 Berlin www.ibu-epd.com
Germany
Author of the Life Cycle Assessment
Ideal Standard International NV +32(0)28004800
Da Vincilaan 2 eboukari@idealstandard.com
1935 Zaventem www.idealstandard.com
Belgium
Owner of the Declaration
Ideal Standard International NV +32(0)28004800
Da Vincilaan 2 eboukari@idealstandard.com
1935 Zaventem www.idealstandard.com
Belgium
8 Environmental Product Declaration - Ideal Standard International - Ceramic Vitreous China product
