ENVIRONMENTAL PRODUCT DECLARATION
as per ISO 14025 and EN 15804+A2
Owner of the Declaration dormakaba International Holding GmbH
Publisher Institut Bauen und Umwelt e.V. (IBU)
Programme holder Institut Bauen und Umwelt e.V. (IBU)
Declaration number EPD-DOR-20240125-CBA1-EN
Issue date 15/07/2024
Valid to 14/07/2029
Kerberos Tripod Barrier-E01
dormakaba
www.ibu-epd.com | https://epd-online.com
General Information
dormakaba Kerberos Tripod Barrier-E01
Programme holder Owner of the declaration
IBU – Institut Bauen und Umwelt e.V. dormakaba International Holding GmbH
Hegelplatz 1 DORMA Platz 1
10117 Berlin 58256 Ennepetal
Germany Germany
Declaration number Declared product / declared unit
EPD-DOR-20240125-CBA1-EN 1 piece of the product: Kerberos Tripod Barrier-E01 consisting of the
following items:
• TPB Drive Unit
• TPB Housing
• Product packaging
This declaration is based on the product category rules: Scope:
Electronic and physical Access Control Systems, 01/08/2021 This Environmental Product Declaration refers to a specific Kerberos
(PCR checked and approved by the SVR) Tripod Barrier-E01 manufactured by dormakaba. The production site is
located in Bühl (Germany).
Issue date Green electricity with Guarantee of Origin (GoO) is being used at this
production site.
15/07/2024
The data represents the year 2024.
The owner of the declaration shall be liable for the underlying information
Valid to
and evidence; the IBU shall not be liable with respect to manufacturer
14/07/2029 information, life cycle assessment data and evidences.
The EPD was created according to the specifications of EN 15804+A2. In
the following, the standard will be simplified as EN 15804.
Verification
The standard EN 15804 serves as the core PCR
Independent verification of the declaration and data according to ISO
14025:2011
internally X externally
Dipl.-Ing. Hans Peters
(Chairman of Institut Bauen und Umwelt e.V.)
Florian Pronold Matthias Klingler,
(Managing Director Institut Bauen und Umwelt e.V.) (Independent verifier)
1 Environmental Product Declaration - dormakaba - Kerberos Tripod Barrier-E01
Product
Performance data of the product with respect to its
Product description/Product definition characteristics in accordance with the relevant technical
Kerberos Tripod barriers can be used for access control. They provision which can be applied are mentioned above.
regulate the flow of people with ease, even during the busiest
periods of the day. dormakaba tripod barriers are compatible
with all types of ID readers and are available in different Base materials/Ancillary materials
designs. In emergencies, designs with collapsible bars in both The major material composition including the packaging of the
directions create an escape route. The tripod barrier bars can product is listed below:
be reset automatically to the normal position by authorized Name Value Unit
personnel as soon as the emergency is over.
Steel 78 %
Paper 11 %
For the Kerberos Tripod Barriers, the standards which can be
applied are the following: Plastics 4 %
Aluminum 4 %
• EN 17352
• EN 50581 Electronics 3 %
• EN 60335-2-103
The Kerberos TPB-E01 includes partial articles which contain
• EN 61000
substances listed in the Candidate List of REACH Regulation
• ISO 9001
1907/2006/EC (date: 23.01.2024) exceeding 0.1 percentage by
• ISO 12100
mass: no
• ISO 13849-1
• ISO 13849-2
The Candidate List can be found on the ECHA website
• 2011/65/EU (RoHS)
address: https:echa.europa.eu/de/home.
• Machinery Directive 2006/42/EG
Reference service life
The CE marking takes into account the proof of conformity with The reference service life of the Kerberos Tripod Barrier-E01
the respective harmonized standards based on the legal amounts to 15 years, depending on the application and
provisions above. frequency of use. For repairs and renewals, suitable spare
parts are available. The Tripod barriers are tested and certified
Application
to EN 17352, meaning they are designed to withstand 4 Mio.
Tripod barriers can be used for access controls and make life
cycles.
easier for reception staff at entrances to office and
administrative buildings, industrial installations, banks,
authorities and many other places.
Technical Data
The Kerberos Tripod Barrier-E01 has following technical
properties:
Name Value Unit
Stainless AISI
Material
Steel 304
Power supply max. 240 VAC
Protection class housing 33 IP
Protection class components conduction
43 IP
supply voltage
LCA: Calculation rules
modules: A4+ A5)
Declared Unit
Production - Module A1-A3
The declared unit is 1 piece of the product: Kerberos Tripod The product stage includes: — A1, raw material extraction,
Barrier-E01 including packaging processing and mechanical treatments, processing of
Name Value Unit secondary material input (e.g. recycling processes), — A2,
transport to the manufacturer, — A3, manufacturing and
Declared unit 1 piece/product
assembly including provision of all materials, products and
Mass of declared product 50.82 kg
energy (green electricity with Guarantee of Origin (GoO)), as
Mass of packaging 7,25 kg
well as waste processing up to the end-of-waste state.
Other declared units are allowed if the conversion is shown
transparently. Construction stage - Modules A4-A5
The construction process stage includes:
— A4, transport to the building site; — A5, installation into the
building; including provision of all materials, products and
System boundary energy, as well as waste processing up to the end-of-waste
The type of EPD is: cradle to gate with options, modules C1– state or disposal of final residues during the construction
C4, and module D (A1–A3 + B6 + C + D and additional process stage.
2 Environmental Product Declaration - dormakaba - Kerberos Tripod Barrier-E01
Use stage - Module B6 Geographic Representativeness
The use stage related to the operation of the building Land or region, in which the declared product system is
includes: — B6, operational energy use manufactured, used or handled at the end of the product´s
lifespan: Global
End-of-life stage– Modules C1-C4 and D
The end-of-life stage includes: — C1, de-construction,
Comparability
demolition: — C2, transport to waste processing; — C3, waste
Basically, a comparison or an evaluation of EPD data is only
processing for reuse, recovery and/or recycling; — C4,
possible if all the data sets to be compared were created
disposal; including provision and all transport, provision of all
according to EN 15804 and the building context, respectively
materials, products and related energy and water use. Module
the product-specific characteristics of performance, are taken
D (Benefits and loads beyond the system boundary) includes:
into account. Background database: GaBi, SP40.
— D, recycling potentials, expressed as net impacts and
benefits.
LCA: Scenarios and additional technical information
End of life (C1-C4)
Characteristic product properties of biogenic carbon
C1: The product dismantling from the building is done manually
without environmental burden.
Name ValueUnit
C2: Transport to waste management is 50 km.
Biogenic carbon content in accompanying kg
2.07 Name Value Unit
packaging C
Collected separately waste type waste type 43.6 kg
Recycling 43.3 kg
Energy recovery 0.2 kg
Landfilling 0.041 kg
Transport to the building site (A4)
Name Value Unit The product is disassembled in a recycling process. Material
recycling is then assumed for metals and electronics. The
Transport distance 100 km
plastic components are assumed to be incinerated with energy
Capacity utilisation (including empty runs) 55 %
recovery. Minor proportions of residues arising from the
Liters of fuel 0,00276 l/100km recycling process are landfilled. Region for the End of Life is:
The product is transported via truck. The main distribution Europe.
region is Europe. In order to allow scaling to a specific point of
installation 100 km is declared. Reuse, recovery and/or recycling potentials (D), relevant
scenario information
Installation into the building (A5) Name Value Unit
Name Value Unit Recycling 100 %
Waste packaging (paper) 5,633 kg The collection rate is 100 %.
Waste packaging (plastic) 1,616 kg
Reference service life
Name Value Unit
Life Span according to the manufacturer 15 a
Operational energy use (B6)
Name Value Unit
Electricity consumption for 1 year 74,095 kWh
Days per year in use 365 days
On mode per day 1 h
Idle mode per day 23 h
On mode power 19 W
Idle mode power 8 W
3 Environmental Product Declaration - dormakaba - Kerberos Tripod Barrier-E01
LCA: Results
DESCRIPTION OF THE SYSTEM BOUNDARY (X = INCLUDED IN LCA; MND = MODULE OR INDICATOR NOT DECLARED; MNR
= MODULE NOT RELEVANT)
Benefits and
Construction loads beyond
Product stage Use stage End of life stage
process stage the system
boundaries
la ire ta m w a Ry lp p u s tro p s n a rT g n iru tc a fu n a M e h t m o rf tro p s n a rTe tis e h t o t e ta g y lb m e s s A e s U e c n a n e tn ia M ria p e R tn e m e c a lp e R tn e m h s ib ru fe R y g re n e la n o ita re p Oe s u re ta w la n o ita re p Oe s u n o itc u rts n o c -e Dn o itilo m e d tro p s n a rT g n is s e c o rp e ts a W la s o p s iD -e s u e R-y re v o c e R-g n ilc y c e Rla itn e to p
A1 A2 A3 A4 A5 B1 B2 B3 B4 B5 B6 B7 C1 C2 C3 C4 D
X X X X X MND X MNR MNR MNR X MND X X X X X
RESULTS OF THE LCA - ENVIRONMENTAL IMPACT according to EN 15804+A2: 1 piece Kerberos TPB-E01
Parameter Unit A1-A3 A4 A5 B2 B6 C1 C2 C3 C4 D
GWP-total kg CO 2 eq 3.14E+02 4.44E-01 1.21E+01 0 4.5E+02 0 1.85E-01 5.08E-01 6.26E-04 -1.62E+02
GWP-fossil kg CO 2 eq 3.2E+02 4.25E-01 4.31E+00 0 4.47E+02 0 1.77E-01 5.08E-01 6.22E-04 -1.63E+02
GWP-
biogenic kg CO 2 eq -6.19E+00 2E-02 7.79E+00 0 1.49E+00 0 8E-03 1.18E-05 2.13E-06 7.09E-01
GWP-luluc kg CO 2 eq 4.52E-01 1.01E-05 3.64E-04 0 6.48E-01 0 4.21E-06 2.87E-05 1.79E-06 -2.97E-01
ODP kg CFC11 eq 5.23E-10 4.49E-17 3.51E-15 0 9.84E-12 0 1.87E-17 2.56E-16 2.31E-18 -9.92E-11
AP mol H+ eq 1.39E+00 4.25E-04 3E-03 0 9.88E-01 0 1.77E-04 9.05E-05 4.46E-06 -7.15E-01
EP-
kg P eq 5.13E-04 9.09E-08 6.12E-07 0 1E-03 0 3.78E-08 4.09E-08 1.07E-09 -1.4E-04
freshwater
EP-marine kg N eq 2.02E-01 1.35E-04 9.73E-04 0 2.19E-01 0 5.63E-05 2.04E-05 1.15E-06 -1.11E-01
EP-terrestrial mol N eq 2.2E+00 2E-03 1.3E-02 0 2.31E+00 0 6.25E-04 4.12E-04 1.26E-05 -1.2E+00
kg NMVOC
POCP 6.09E-01 3.83E-04 3E-03 0 6.01E-01 0 1.59E-04 5.65E-05 3.48E-06 -3.28E-01
eq
ADPE kg Sb eq 1.33E-02 1.27E-08 5.12E-08 0 1.3E-04 0 5.3E-09 3.52E-09 5.59E-11 -5E-03
ADPF MJ 4.19E+03 6.02E+00 4.43E+00 0 7.87E+03 0 2.51E+00 2.36E-01 8E-03 -2.03E+03
m3 world eq
WDP 8.82E+01 8.32E-04 1.41E+00 0 9.75E+01 0 3.46E-04 5.2E-02 6.52E-05 -6.17E+01
deprived
GWP = Global warming potential; ODP = Depletion potential of the stratospheric ozone layer; AP = Acidification potential of land and water; EP =
Eutrophication potential; POCP = Formation potential of tropospheric ozone photochemical oxidants; ADPE = Abiotic depletion potential for non-fossil
resources; ADPF = Abiotic depletion potential for fossil resources; WDP = Water (user) deprivation potential)
RESULTS OF THE LCA - INDICATORS TO DESCRIBE RESOURCE USE according to EN 15804+A2: 1 piece Kerberos TPB-E01
Parameter Unit A1-A3 A4 A5 B2 B6 C1 C2 C3 C4 D
PERE MJ 9.86E+02 1.9E-02 6.85E+01 0 3.49E+03 0 8E-03 6.1E-02 1E-03 -4.8E+02
PERM MJ 6.76E+01 0 -6.76E+01 0 0 0 0 0 0 0
PERT MJ 1.05E+03 1.9E-02 9.53E-01 0 3.49E+03 0 8E-03 6.1E-02 1E-03 -4.8E+02
PENRE MJ 4.12E+03 6.03E+00 7.39E+01 0 7.87E+03 0 2.51E+00 7.99E+00 8E-03 -2.03E+03
PENRM MJ 7.72E+01 0 -6.95E+01 0 0 0 0 -7.76E+00 0 0
PENRT MJ 4.2E+03 6.03E+00 4.43E+00 0 7.87E+03 0 2.51E+00 2.36E-01 8E-03 -2.03E+03
SM kg 2.25E+01 0 0 0 0 0 0 0 0 0
RSF MJ 0 0 0 0 0 0 0 0 0 0
NRSF MJ 0 0 0 0 0 0 0 0 0 0
FW m3 3.43E+00 3.41E-05 3.3E-02 0 4.03E+00 0 1.42E-05 1E-03 2.06E-06 -2.55E+00
PERE = Use of renewable primary energy excluding renewable primary energy resources used as raw materials; PERM = Use of renewable primary
energy resources used as raw materials; PERT = Total use of renewable primary energy resources; PENRE = Use of non-renewable primary energy
excluding non-renewable primary energy resources used as raw materials; PENRM = Use of non-renewable primary energy resources used as raw
materials; PENRT = Total use of non-renewable primary energy resources; SM = Use of secondary material; RSF = Use of renewable secondary fuels;
NRSF = Use of non-renewable secondary fuels; FW = Use of net fresh water
RESULTS OF THE LCA – WASTE CATEGORIES AND OUTPUT FLOWS according to EN 15804+A2:
1 piece Kerberos TPB-E01
Parameter Unit A1-A3 A4 A5 B2 B6 C1 C2 C3 C4 D
HWD kg 2.03E-05 5.85E-10 1.1E-08 0 3.26E-06 0 2.43E-10 8.98E-10 1.24E-10 2.46E-07
NHWD kg 2.52E+01 6.17E-04 6.77E-01 0 5.58E+00 0 2.56E-04 5.3E-02 4.1E-02 -1.79E+01
RWD kg 6.2E-02 6.47E-06 2.03E-04 0 1.19E+00 0 2.69E-06 8.75E-06 9.29E-08 -3.4E-02
CRU kg 0 0 0 0 0 0 0 0 0 0
MFR kg 0 0 0 0 0 0 0 4.2E+01 0 0
MER kg 0 0 0 0 0 0 0 0 0 0
EEE MJ 0 0 1.97E+01 0 0 0 0 1.17E+00 0 0
4 Environmental Product Declaration - dormakaba - Kerberos Tripod Barrier-E01
EET MJ 0 0 3.94E+01 0 0 0 0 2.68E+00 0 0
HWD = Hazardous waste disposed; NHWD = Non-hazardous waste disposed; RWD = Radioactive waste disposed; CRU = Components for re-use;
MFR = Materials for recycling; MER = Materials for energy recovery; EEE = Exported electrical energy; EET = Exported thermal energy
RESULTS OF THE LCA – additional impact categories according to EN 15804+A2-optional:
1 piece Kerberos TPB-E01
Parameter Unit A1-A3 A4 A5 B2 B6 C1 C2 C3 C4 D
Disease
PM 2.16E-05 2.24E-09 2.17E-08 0 8.29E-06 0 9.3E-10 1.16E-09 5.52E-11 -1.42E-05
incidence
IR kBq U235 eq 7.72E+00 9.25E-04 2.7E-02 0 1.96E+02 0 3.85E-04 7.88E-04 9.56E-06 -5.96E+00
ETP-fw CTUe 2.23E+03 4.27E+00 1.91E+00 0 3.36E+03 0 1.78E+00 8.8E-02 5E-03 -1.04E+03
HTP-c CTUh 4.73E-05 8.03E-11 1.25E-10 0 9.29E-08 0 3.34E-11 7.66E-12 6.91E-13 -3.14E-07
HTP-nc CTUh 5.15E-06 3.44E-09 9.01E-09 0 3.42E-06 0 1.43E-09 7.75E-10 7.62E-11 -8.44E-07
SQP SQP 1.59E+03 1.5E-02 1.24E+00 0 2.51E+03 0 6E-03 7.1E-02 2E-03 -2.79E+02
PM = Potential incidence of disease due to PM emissions; IR = Potential Human exposure efficiency relative to U235; ETP-fw = Potential comparative
Toxic Unit for ecosystems; HTP-c = Potential comparative Toxic Unit for humans (cancerogenic); HTP-nc = Potential comparative Toxic Unit for humans
(not cancerogenic); SQP = Potential soil quality index
Disclaimer 1 – for the indicator “Potential Human exposure efficiency relative to U235”. This impact category deals mainly with the
eventual impact of low-dose ionizing radiation on human health of the nuclear fuel cycle. It does not consider effects due to possible
nuclear accidents, occupational exposure or radioactive waste disposal in underground facilities. Potential ionizing radiation from the
soil, radon and from some construction materials is also not measured by this indicator.
Disclaimer 2 – for the indicators “abiotic depletion potential for non-fossil resources”, “abiotic depletion potential for fossil resources”,
“water (user) deprivation potential, deprivation-weighted water consumption”, “potential comparative toxic unit for ecosystems”,
“potential comparative toxic unit for humans – cancerogenic”, “Potential comparative toxic unit for humans - not cancerogenic”,
“potential soil quality index”. The results of this environmental impact indicator shall be used with care as the uncertainties on these
results are high as there is limited experience with the indicator.
This EPD was created using a software tool.
References
EN 17352
EN 17352:2022 REACH
Power operated pedestrian entrance control equipment - Safety Regulation (EC) No 1907/2006 of the European Parliament and
in use - Requirements of the Council on the Registration, Evaluation, Authorisation
and Restriction of Chemicals (REACH)
EN 50581
EN 50581:2013-02 RoHS
Technical documentation for the assessment 2011/65/EU, Directive on the restriction of the use of certain
of electrical and electronic products with respect to the hazardous substances in electrical and electronic equipment
restriction of hazardous substances
EN 60335-2 Further References
EN 60335-2-103: 2016-05
Household and similar electrical appliances EN 15804
EN 15804+A2:2019+AC:2021,
ECHA Sustainability of construction works — Environmental Product
European Chemical Agency Declarations — Core rules for the product category of
construction products
ISO 9001
ISO 9001: 2015-09 IBU 2021
Quality management systems requirements General Instructions for the EPD programme of Institut Bauen
und Umwelt e.V. Version 2.0, Berlin: Institut Bauen und Umwelt
ISO 12100 e.V., 2021. www.ibu-epd.com
ISO 12100: 2010
Safety of machinery ISO 14025
ISO 14025:2011-10, Environmental
ISO 13849-1 labels and declarations — Type III environmental declarations
ISO 13849-1: 2016-06 — Principles and procedures
Safety of machinery
GaBi
ISO 13849-2 Sphera Solutions GmbH
ISO 13849-2: 2013-02 Gabi Software System and Database for Life Cycle Engineering
Safety of machinery 19922020
Version 10.0.0.71
Machinery Directive 2006/42/EC University of Stuttgart
Directive 2006/42/EC of the European Parliament and of the Leinfelden-Echterdingen
council of 17 May 2006 on machinery, and amending Directive
95/16/EC GaBi ts documentation
5 Environmental Product Declaration - dormakaba - Kerberos Tripod Barrier-E01
GaBi life cycle inventory data documentation 15804+A2:2019, Version 1.0, 2020, Institut Bauen und Umwelt
(https://www.gabisoftware.com/support/gabi/gabidatabase- e.V., www.ibu-epd.com.
2020-lcidocumentation/).
PCR Part B
LCA-tool dormakaba PCR – Part B: Requirements on the EPD for Electronic and
Tool No.: IBU-DOR-202109-LT1-EN. physical Access Control Systems, version 08/2021, Institut
Developed by Sphera Solutions GmbH Bauen und Umwelt e.V., www.ibu-epd.com.
PCR Part A
PCR – Part A: Calculation Rules for the Life Cycle Assessment
and Requirements on the Project Re-port according to EN
6 Environmental Product Declaration - dormakaba - Kerberos Tripod Barrier-E01
Publisher
Institut Bauen und Umwelt e.V. +49 (0)30 3087748- 0
Hegelplatz 1 info@ibu-epd.com
10117 Berlin www.ibu-epd.com
Germany
Programme holder
Institut Bauen und Umwelt e.V. +49 (0)30 3087748- 0
Hegelplatz 1 info@ibu-epd.com
10117 Berlin www.ibu-epd.com
Germany
Author of the Life Cycle Assessment
dormakaba International Holding GmbH +49 2333 793-0
DORMA Platz 1 info.de@dormakaba.com
58256 Ennepetal www.dormakaba.com
Germany
Owner of the Declaration
dormakaba International Holding GmbH +49 2333 793-0
DORMA Platz 1 info.de@dormakaba.com
58256 Ennepetal www.dormakaba.com
Germany
7 Environmental Product Declaration - dormakaba - Kerberos Tripod Barrier-E01
