ENVIRONMENTAL PRODUCT DECLARATION
as per ISO 14025 and EN 15804+A2
Owner of the Declaration Kingspan Insulation B.V.
Publisher Institut Bauen und Umwelt e.V. (IBU)
Programme holder Institut Bauen und Umwelt e.V. (IBU)
Declaration number EPD-KSI-20230321-CBA1-EN
Issue date 22.09.2023
Valid to 21.09.2028
Kooltherm® K20
Kingspan Insulation B.V.
www.ibu-epd.com | https://epd-online.com
General Information
Kingspan Insulation B.V. Kooltherm® K20
Programme holder Owner of the declaration
IBU – Institut Bauen und Umwelt e.V. Kingspan Insulation B.V.
Hegelplatz 1 Lingewei 8
10117 Berlin 4004LL Tiel
Germany Netherlands
Declaration number Declared product / declared unit
EPD-KSI-20230321-CBA1-EN Kooltherm® K20 Concrete Sandwich Board
1 m², 80 mm thickness, R = 3,80 m²·K/W
D
This declaration is based on the product category rules: Scope:
Insulating materials made of foam plastics, 01.08.2021 The insulation material Kooltherm® K20 is produced by Kingspan
(PCR checked and approved by the SVR) Insulation B.V. at the manufacturing facilities in Tiel, the Netherlands and
Jönköping, Sweden. This EPD is based on weighted averages which have
been determined on the basis of the single values originating from the
Issue date different Kingspan Insulation factories.
22.09.2023
Kooltherm® K20 is a rigid thermoset cellular insulation material faced on
both sides with a glass tissue based facing.
Valid to
In order to enable the user of the EPD to calculate the LCA results for
21.09.2028 different thicknesses, the EPD contains the respective calculation rules.
The owner of the declaration shall be liable for the underlying information
and evidence; the IBU shall not be liable with respect to manufacturer
information, life cycle assessment data and evidences.
The EPD was created according to the specifications of EN 15804+A2. In
the following, the standard will be simplified as EN 15804.
Verification
The standard EN 15804 serves as the core PCR
Dipl.-Ing. Hans Peters Independent verification of the declaration and data according to ISO
(Chairman of Institut Bauen und Umwelt e.V.) 14025:2011
internally X externally
Florian Pronold Vito D'Incognito,
(Managing Director Institut Bauen und Umwelt e.V.) (Independent verifier)
1 Environmental Product Declaration - Kingspan Insulation B.V. - Kooltherm® K20
Product
creep (not placed under permanent load).
Product description/Product definition
Kooltherm® K20 is a rigid thermoset cellular insulation material Performance data of the product in accordance with the
faced on both sides with a glass tissue based facing. The declaration of performance with respect to its essential
product is available in variable thicknesses from 20 mm up to characteristics according to EN 13166 - Thermal insulation
160 mm. This EPD is based on a thickness of 80 mm and products for buildings - Factory made phenolic foam (PF)
R -value of 3,80 m²·K/W. products - Specification
D
Base materials/Ancillary materials
For the placing on the market of the product in the European
The main materials are phenolic (PF) resin (between 70-80%)
Union/European Free Trade Association (EU/EFTA) (with the
with added catalyst and additives (between 15-20%). Phenolic
exception of Switzerland) Regulation (EU) No. 305/2011 (CPR)
rigid foam onto a facing material (between 5-10%) is formed by
applies. The product needs a declaration of performance taking
the chemical reaction of these materials and adding a blowing
into consideration EN 13166 - Thermal insulation products for
agent with no ozone depletion potential (ca. 5%). Due to the
buildings - Factory made phenolic foam (PF) products -
closed-cell structure (conform EN 13166), the blowing agent
specification and the CE-marking. For the application and use
remains in the foam. In the current REACH regulations,
the respective national provisions apply.
phenolic foam insulation products are considered 'articles' and
Application are exempt from the requirements of Article 57 and 59(1) of
Kooltherm® K20 is suitable for use as insulation for concrete REACH Regulation (EC) No 1907/2006. These products are
not classified as 'hazardous products' according to any current
wall systems.
legislation, and can hence be declared as follows:
Technical Data - This article contains substances listed in the candidate list
The declaration of performance of the product can be found at (date: 17.01.2023) exceeding 0.1 percentage by mass: no.
www.kingspan.com. - This article contains other carcinogenic, mutagenic, reprotoxic
(CMR) substances in categories 1A or 1B which are not on the
Constructional data
candidate list, exceeding 0.1 percentage by mass: no.
Name Value Unit - Biocide products were added to this construction products or it
Compressive strength acc. to EN 13166 ≥ 100 kPa has been treated with biocide products (this then concerns a
Tensile strength perpendicular to faces acc. to treated product as defined by the (EU) Biocidal Products
≥ 60 kPa
EN 13166 Regulation No. 528/2012 (BPR): no.
Thermal conductivity λd acc. to EN 13166 for d
0.021W/(mK) The chemical functional group of the additives used in the resin
= 20 – 160 mm
is that of non-ionic surfactants.
Thermal conductivity λd acc. to EN 13166 for d
0.021W/(mK)
= 160 – 200 mm (double layers) Reference service life
Technical parameters not included are modulus of elasticity as The reference service life is not to be declared in this EPD as it
well as sound absorption (not relevant for this application) and does not cover the use stage.
LCA: Calculation rules
Type of EPD: according to EN 15804: cradle to gate with
Declared Unit options, modules C1–C4, and module D (A1–A3, C, D and
The declared unit (1 m²) and conversion factors are listed in the additional modules: A4,A5).
table below.
Declared unit The product stage is a mandatory information module and it
covers:
Name Value Unit
· A1, raw material extraction and processing, processing of
Declared unit 1 m2 secondary material input (e.g. recycling processes),
Gross density (foam) 35 kg/m3 · A2, transport to the manufacturer,
Grammage 2.94 kg/m2 · A3, manufacturing, including provision of all materials,
products and energy, packaging processing and its transport,
Layer thickness 0.08 m
as well as waste processing up to the end-of-waste state or
This EPD is based on a weighted average of the annual disposal of final residues during the product stage.
production volume of two factories producing the products
Kooltherm® K20. The scope of this EPD is the thermal The construction process stage includes:
insulation product Kooltherm® K20 as produced by Kingspan · A4 transport to the building site;
Insulation at the manufacturing facilities in Tiel (the · A5 installation in the building including provision of all
Netherlands), Jönköping (Sweden). The environmental impacts materials, products and energy, as well as waste processing up
have been calculated per plant over the calendar year 2022. to the end-of-waste state or disposal of final residues during the
Based on the one-year production volume of Kooltherm® K20 construction process stage.
per plant, the individual environmental impacts are weighted.
The end-of-life stage is a mandatory information module and it
The EPD is studied for a common product thickness of 80mm. covers:
Multiplication factors are included to calculate impacts for other · C1 de-construction, demolition;
product thicknesses within the range of 20 to 160 mm. · C2 transport to waste processing;
· C3 waste processing for reuse, recovery and/or recycling;
System boundary · C4 disposal (not applicable for this EPD) including provision
2 Environmental Product Declaration - Kingspan Insulation B.V. - Kooltherm® K20
and all transport, provision of all materials, products and related product
energy and water use. at the end-of-life stage are assigned to the product system
(C3); resulting potential credits for thermal and electrical energy
Environmental burden of the incineration (R1 > 60%) of the from energy substitution are declared in module D.
Factors for different thicknesses Geographic Representativeness
The LCA results for the insulation material declared in this EPD Land or region, in which the declared product system is
refer to a product with a thickness of 80 mm. To enable the user manufactured, used or handled at the end of the product´s
of the EPD to calculate the results for different thicknesses the lifespan: Europe
factors in the following table can be used for the calculation.
The LCA results in chapter 5 have to be multiplied by these
Comparability
factors. The scaling factors are applicable for the complete
Basically, a comparison or an evaluation of EPD data is only
product, where the facings are for all product thicknesses
possible if all the data sets to be compared were created
equal, and the foam inputs are scaling upwards and
according to EN 15804 and the building context, respectively
downwards with other product thicknesses.
the product-specific characteristics of performance, are taken
into account.
Background data from GaBi ts Version 10 is used with GaBi
data sets CUP2022.1
LCA: Scenarios and additional technical information
Installation into the building (A5)
Characteristic product properties of biogenic carbon
The total mass of biogenic carbon containing materials is less Name ValueUnit
than 5 % of the total mass of the product and accompanying Output substances following waste treatment on
0.06 kg
packaging. site packaging material
Technical information
The recycling of the packaging is considered in A5.
The following technical information is a basis for the declared
modules or can be used for developing specific scenarios in the
context of a building assessment. End of life (C1-C4)
The assumptions for C1 are: diesel driven excavator (100 kW;
Manufacturing (A3) 0.2 litre fuel per ton excavated material).
Within A1-A3 the following packaging of the final product is The assumptions for C2 are: Truck Euro 6, diesel driven, 26-28
included: t gross weight, assumed distance 50 km
Polyethylene cover and wrap: 0,05 kg/m² Name Value Unit
Others (mainly Expanded Polystyrene skid): 0,01 kg/m²
Collected as mixed construction waste 2.94 kg
Energy recovery 2.94 kg
Transport to the building site (A4)
R1-value of waste incineration plant >60 %
Name Value Unit
Litres of fuel 0.0103 l/100km
Transport distance 100 km Reuse, recovery and/or recycling potentials (D), relevant
Grammage of products transported 2,94 kg/m2 scenario information
Waste incineration with energy recuperation is assumed as
end-of-life scenario.
3 Environmental Product Declaration - Kingspan Insulation B.V. - Kooltherm® K20
LCA: Results
DESCRIPTION OF THE SYSTEM BOUNDARY (X = INCLUDED IN LCA; ND = MODULE OR INDICATOR NOT DECLARED; MNR =
MODULE NOT RELEVANT)
Benefits and
Construction loads beyond
Product stage Use stage End of life stage
process stage the system
boundaries
la ire ta m w a Ry lp p u s tro p s n a rT g n iru tc a fu n a M e h t m o rf tro p s n a rTe tis e h t o t e ta g y lb m e s s A e s U e c n a n e tn ia M ria p e R tn e m e c a lp e R tn e m h s ib ru fe R y g re n e la n o ita re p Oe s u re ta w la n o ita re p Oe s u n o itc u rts n o c -e Dn o itilo m e d tro p s n a rT g n is s e c o rp e ts a W la s o p s iD -e s u e R-y re v o c e R-g n ilc y c e Rla itn e to p
A1 A2 A3 A4 A5 B1 B2 B3 B4 B5 B6 B7 C1 C2 C3 C4 D
X X X X X MND MND MNR MNR MNR MND MND X X X X X
RESULTS OF THE LCA - ENVIRONMENTAL IMPACT according to EN 15804+A2: 1 m2 80 mm thickness
Parameter Unit A1-A3 A4 A5 C1 C2 C3 C4 D
GWP-total kg CO 2 eq 5.56E+00 2.47E-02 1.5E-01 1.89E-03 1.24E-02 6.43E+00 0 -2.54E+00
GWP-fossil kg CO 2 eq 5.54E+00 2.46E-02 1.5E-01 1.88E-03 1.23E-02 6.43E+00 0 -2.52E+00
GWP-biogenic kg CO 2 eq -3.84E-02 -3.41E-05 8.17E-06 2.52E-06 -1.7E-05 4.37E-04 0 -1.29E-02
GWP-luluc kg CO 2 eq 6.38E-02 1.37E-04 1.77E-06 2.32E-08 6.87E-05 1.14E-05 0 -2.78E-04
ODP kg CFC11 eq 1.14E-08 1.48E-15 2.66E-14 1.16E-16 7.39E-16 4.7E-13 0 -1.71E-11
AP mol H+ eq 1.13E-02 2.54E-05 1.86E-05 8.75E-06 1.27E-05 3.79E-03 0 -3.33E-03
EP-freshwater kg P eq 1.87E-05 7.36E-08 6.73E-09 3.8E-10 3.68E-08 1.27E-07 0 -3.48E-06
EP-marine kg N eq 3.18E-03 8.31E-06 5E-06 4.17E-06 4.16E-06 1.84E-03 0 -9.01E-04
EP-terrestrial mol N eq 3.16E-02 9.89E-05 8.48E-05 4.57E-05 4.95E-05 2.11E-02 0 -9.65E-03
kg NMVOC
POCP 1.66E-02 2.24E-05 1.44E-05 1.18E-05 1.12E-05 4.71E-03 0 -2.52E-03
eq
ADPE kg Sb eq 5.76E-06 2.06E-09 6.5E-10 7.71E-11 1.03E-09 1.3E-08 0 -3.82E-07
ADPF MJ 1.61E+02 3.29E-01 5.52E-02 2.55E-02 1.65E-01 1.66E+00 0 -4.29E+01
m3 world eq
WDP 8.79E-01 2.21E-04 1.42E-02 3.5E-06 1.11E-04 6.33E-01 0 -2.7E-01
deprived
GWP = Global warming potential; ODP = Depletion potential of the stratospheric ozone layer; AP = Acidification potential of land and water; EP =
Eutrophication potential; POCP = Formation potential of tropospheric ozone photochemical oxidants; ADPE = Abiotic depletion potential for non-fossil
resources; ADPF = Abiotic depletion potential for fossil resources; WDP = Water (user) deprivation potential)
RESULTS OF THE LCA - INDICATORS TO DESCRIBE RESOURCE USE according to EN 15804+A2: 1 m2 80 mm thickness
Parameter Unit A1-A3 A4 A5 C1 C2 C3 C4 D
PERE MJ 2.06E+01 1.87E-02 1.42E-02 9.63E-05 9.36E-03 2.89E-01 0 -1.18E+01
PERM MJ 0 0 0 0 0 0 0 0
PERT MJ 2.06E+01 1.87E-02 1.42E-02 9.63E-05 9.36E-03 2.89E-01 0 -1.18E+01
PENRE MJ 7.88E+01 3.3E-01 2.6E+00 2.55E-02 1.65E-01 8.19E+01 0 -4.29E+01
PENRM MJ 8.27E+01 0 -2.55E+00 0 0 -8.02E+01 0 0
PENRT MJ 1.62E+02 3.3E-01 5.53E-02 2.55E-02 1.65E-01 1.66E+00 0 -4.29E+01
SM kg 0 0 0 0 0 0 0 0
RSF MJ 0 0 0 0 0 0 0 0
NRSF MJ 0 0 0 0 0 0 0 0
FW m3 3.5E-02 2.12E-05 3.37E-04 1.45E-07 1.06E-05 1.49E-02 0 -1.14E-02
PERE = Use of renewable primary energy excluding renewable primary energy resources used as raw materials; PERM = Use of renewable primary
energy resources used as raw materials; PERT = Total use of renewable primary energy resources; PENRE = Use of non-renewable primary energy
excluding non-renewable primary energy resources used as raw materials; PENRM = Use of non-renewable primary energy resources used as raw
materials; PENRT = Total use of non-renewable primary energy resources; SM = Use of secondary material; RSF = Use of renewable secondary fuels;
NRSF = Use of non-renewable secondary fuels; FW = Use of net fresh water
RESULTS OF THE LCA – WASTE CATEGORIES AND OUTPUT FLOWS according to EN 15804+A2:
1 m2 80 mm thickness
Parameter Unit A1-A3 A4 A5 C1 C2 C3 C4 D
HWD kg 7.65E-05 1.58E-12 4.6E-12 8.44E-14 7.91E-13 2.29E-10 0 -5.81E-09
NHWD kg 8.67E-02 4.73E-05 1.34E-02 2.39E-06 2.37E-05 3.23E-02 0 -2.17E-02
RWD kg 1.84E-03 4.07E-07 2.3E-06 2.8E-08 2.03E-07 6.85E-05 0 -3.39E-03
CRU kg 0 0 0 0 0 0 0 0
MFR kg 0 0 0 0 0 0 0 0
MER kg 0 0 5.99E-02 0 0 2.91E+00 0 0
EEE MJ 0 0 2.72E-01 0 0 1.11E+01 0 0
EET MJ 0 0 4.86E-01 0 0 1.99E+01 0 0
HWD = Hazardous waste disposed; NHWD = Non-hazardous waste disposed; RWD = Radioactive waste disposed; CRU = Components for re-use;
MFR = Materials for recycling; MER = Materials for energy recovery; EEE = Exported electrical energy; EET = Exported thermal energy
4 Environmental Product Declaration - Kingspan Insulation B.V. - Kooltherm® K20
RESULTS OF THE LCA – additional impact categories according to EN 15804+A2-optional:
1 m2 80 mm thickness
Parameter Unit A1-A3 A4 A5 C1 C2 C3 C4 D
Disease
PM 1.16E-07 1.47E-10 2.27E-10 9.91E-11 7.33E-11 1.05E-08 0 -2.75E-08
incidence
IR kBq U235 eq 2.83E-01 5.96E-05 3.16E-04 4.08E-06 2.98E-05 1.1E-02 0 -5.74E-01
ETP-fw CTUe 5.98E+01 2.29E-01 3.95E-02 1.77E-02 1.14E-01 5.66E-01 0 -9.45E+00
HTP-c CTUh 2.73E-09 4.61E-12 2.22E-12 3.28E-13 2.31E-12 4.28E-11 0 -4.33E-10
HTP-nc CTUh 8.59E-08 2.39E-10 2.24E-10 1.66E-11 1.2E-10 1.55E-09 0 -1.66E-08
SQP SQP 1.08E+01 1.13E-01 1.41E-02 7.03E-05 5.67E-02 3.47E-01 0 -7.68E+00
PM = Potential incidence of disease due to PM emissions; IR = Potential Human exposure efficiency relative to U235; ETP-fw = Potential comparative
Toxic Unit for ecosystems; HTP-c = Potential comparative Toxic Unit for humans (cancerogenic); HTP-nc = Potential comparative Toxic Unit for humans
(not cancerogenic); SQP = Potential soil quality index
Disclaimer 1 – for the indicator IR
This impact category deals mainly with the eventual impact of low dose ionizing radiation on human health of the nuclear fuel cycle. It
does not consider effects due to possible nuclear accidents, occupational exposure nor due to radioactive waste disposal in
underground facilities. Potential ionizing radiation from the soil, from radon and from some construction materials is also not measured
by this indicator.
Disclaimer 2 – for the indicators ADPE, ADPF, WDP, ETP-fw, HTP-c, HTP-nc, SQP
The results of this environmental impact indicator shall be used with care as the uncertainties on these results are high or as there is
limited experienced with the indicator. This EPD was created using a software tool.
References
EN 13166 ISO 14025
EN 13166:2012+A2:2016: Thermal insulation products EN ISO 14025:2011-10 - Environmental labels and declarations
for buildings. Factory made phenolic foam (PF) — Type III environmental declarations — Principles and
products. Specification procedures
EN 15804+A2 LCA-tool
EN15804/A2: Sustainability of construction works - Kingspan LCA tool, version 1.2. IBU-KSI-202001-LT1-EN.
Environmental product declarations - Core rules for the Developed by Sphera Solutions GmbH (formely Thinkstep
product category of construction products, 2019 GmbH)
BPR PCR Version 1.7, Part A
Regulation (EU) No 528/2012 of the European Parliament and Institut Bauen und Umwelt e.V., Berlin (pub.): Product Category
of the Council of 22 May 2012 concerning the making available Rules for Building-Related Products andservices, Part A:
on the market and use of biocidal products Calculation Rules for the Life Cycle Assessment and
Requirements on the Project Report according to EN
15804+A2:2019 November 2021
CPR
Regulation (EU) No. 305/2011 of the European
Parliament and of the Council of 9 March 2011 laying PCR, Part B
down harmonised condition for the marketing of Institut Bauen und Umwelt e.V., Berlin (pub.): Product Category
construction products and repealing Council Directive Rules for Construction Products from the range of
89/106/EC Environmental Product Declarations of Institut Bauen und
Umwelt (IBU), Part B: Requirements on the EPD for insulating
materials made of foam plastics. June 2023
GaBi ts
thinkstep AG: Leinfelden-Echterdingen GaBi Software-System
and Database for Life Cycle Engineering 1992-2019 REACH
Regulation (EC) No 1907/2006 of the European Parliament and
of the Council on the Registration, Evaluation, Authorisation
IBU 2021 and Restriction of Chemicals (REACH)
Institut Bauen und Umwelt e.V.: General Instructions for the https://echa.europa.eu/candidate-list-table; accessed 17th of
EPD programme of Institut Bauen und Umwelte.V., Version 2.0, January 2023, 233 substances listed.
Berlin: Institut Bauen und Umwelte.V., 2021. www.ibu-epd.com
5 Environmental Product Declaration - Kingspan Insulation B.V. - Kooltherm® K20
Publisher
Institut Bauen und Umwelt e.V. +49 (0)30 3087748- 0
Hegelplatz 1 info@ibu-epd.com
10117 Berlin www.ibu-epd.com
Germany
Programme holder
Institut Bauen und Umwelt e.V. +49 (0)30 3087748- 0
Hegelplatz 1 info@ibu-epd.com
10117 Berlin www.ibu-epd.com
Germany
Author of the Life Cycle Assessment
Kingspan Insulation B.V. +31 (0) 543 543 210
Lingewei 8 info@kingspaninsulation.nl
4004LL Tiel www.kingspan.com
Netherlands
Owner of the Declaration
Kingspan Insulation B.V. +31 (0) 543 543 210
Lingewei 8 info@kingspaninsulation.nl
4004LL Tiel www.kingspan.com
Netherlands
6 Environmental Product Declaration - Kingspan Insulation B.V. - Kooltherm® K20
