ENVIRONMENTAL PRODUCT DECLARATION
as per ISO 14025 and EN 15804+A2
Owner of the Declaration Kingspan Insulation B.V.
Publisher Institut Bauen und Umwelt e.V. (IBU)
Programme holder Institut Bauen und Umwelt e.V. (IBU)
Declaration number EPD-KSI-20230318-CBA1-EN
Issue date 22.09.2023
Valid to 21.09.2028
Kooltherm® K15 C
Kingspan Insulation BV
www.ibu-epd.com | https://epd-online.com
General Information
Kingspan Insulation BV Kooltherm® K15 C
Programme holder Owner of the declaration
IBU – Institut Bauen und Umwelt e.V. Kingspan Insulation B.V.
Hegelplatz 1 Lingewei 8
10117 Berlin 4004LL Tiel
Germany Netherlands
Declaration number Declared product / declared unit
EPD-KSI-20230318-CBA1-EN Kooltherm® K15 C Facades Board,
1 m², 80 mm thickness, R = 3,80 m²·K/W
D
This declaration is based on the product category rules: Scope:
Insulating materials made of foam plastics, 01.08.2021 The insulation material Kooltherm® K15C is produced by Kingspan
(PCR checked and approved by the SVR) Insulation B.V. at the manufacturing facility in Jönköping, Sweden.
Kooltherm® K15C is a rigid thermoset cellular insulation material faced
Issue date with a micro-perforated reinforced aluminum foil on the outer side and a
22.09.2023 mineral coated glass tissue on the inner side.
In order to enable the user of the EPD to calculate the LCA results for
Valid to different thicknesses, the EPD contains the respective calculation rules.
21.09.2028 The owner of the declaration shall be liable for the underlying information
and evidence; the IBU shall not be liable with respect to manufacturer
information, life cycle assessment data and evidences.
The EPD was created according to the specifications of EN 15804+A2. In
the following, the standard will be simplified as EN 15804.
Verification
The standard EN 15804 serves as the core PCR
Independent verification of the declaration and data according to ISO
14025:2011
Dipl.-Ing. Hans Peters
internally X externally
(Chairman of Institut Bauen und Umwelt e.V.)
Florian Pronold Vito D'Incognito,
(Managing Director Institut Bauen und Umwelt e.V.) (Independent verifier)
1 Environmental Product Declaration - Kingspan Insulation BV - Kooltherm® K15 C
Product
Performance data of the product in accordance with the
Product description/Product definition declaration of performance with respect to its essential
The Kooltherm® K15C is a rigid thermoset cellular insulation characteristics according to EN 13166 - Thermal insulation
material faced with a micro-perforated reinforced aluminum foil products for buildings - Factory made phenolic foam (PF)
on the outer side and a mineral coated glass tissue on the inner products - Specification.
side. The product is available in variable thicknesses from 50
mm up to 160 mm. This EPD is based on a thickness of 80 mm Base materials/Ancillary materials
and RD-value of 3,80 m²·K/W. The main materials are phenolic (PF) resin (between 70-80%)
with added catalyst and additives (between 15-20%). Phenolic
For the placing on the market of the product in the European rigid foam onto a facing material (between 5-10%) is formed by
Union/European Free Trade Association (EU/EFTA) (with the the
exception of Switzerland) Regulation (EU) No. 305/2011 CPR chemical reaction of these materials and adding a blowing
applies. The product needs a declaration of performance taking agent with no ozone depletion potential (ca. 5%).
into consideration EN 13166 - Thermal insulation products for
buildings - Factory made phenolic foam (PF) products - In the current REACH regulations, phenolic foam insulation
Specification and the CE-marking. For the application and use products are considered 'articles' and are exempt from the
the respective national provisions apply. requirements of Article 57 and 59(1) of REACH Regulation (EC)
No 1907/2006. These products are not classified as 'hazardous
Application products' according to any current legislation, and can hence
Kooltherm® K15 C is suitable for use as insulation for ventilated be declared as follows:
facades in both new and renovation construction and also on
concrete element in semi-sandwich constructions. - This article contains substances listed in the candidate list
(date: 17.01.2023) exceeding 0.1 percentage by mass: no.
Technical Data - This article contains other carcinogenic, mutagenic, reprotoxic
The declaration of performance of the product can be found at (CMR) substances in categories 1A or 1B which are not on the
www.kingspan.com. candidate list, exceeding 0.1 percentage by mass: no.
Constructional data - Biocide products were added to this construction product or it
has been treated with biocide products (this then concerns a
Name Value Unit
treated product as defined by the (EU) Biocide Products
Compressive strength acc. to EN 13166 ≥ 100 kPa Regulation No. 528/2012 (BPR): no.'
Thermal conductivity λd acc. to /EN 13166/ for d
0.021W/(mK)
= 50-160mm The chemical functional group of the additives used in the resin
is that of non-ionic surfactants.
Technical parameters not included are modulus of elasticity as
well as sound absorption (not relevant for this application) and
Reference service life
creep (not placed under permanent load). See Declaration of
The reference service life is not to be declared in this EPD as it
Performance for further information.
does not cover the use stage.
LCA: Calculation rules
The product stage is a mandatory information module and it
Declared Unit covers:
The declared unit (1 m²) and conversion factors are listed in the - A1, raw material extraction and processing, processing of
table below. secondary material input (e.g. recycling processes)
Declared unit - A2, transport to the manufacturer
- A3, manufacturing, including the provision of all materials,
Name Value Unit
products and energy, packaging processing and its transport,
Declared unit 1 m2 as well as waste processing up to the end-of waste state or
Gross density (foam) 35 kg/m3 disposal of final residues during the product stage.
Grammage 3.035 kg/m2
The construction process stage includes:
Layer thickness 0.08 m
- A4 transport to the building site;
The scope of this EPD is the thermal insulation product - A5 installation in the building including provision of all
Kooltherm® K15 C as produced by Kingspan Insulation at the materials, products and energy, as well as waste processing up
manufacturing facility in Jönköping (Sweden). The to the end-of-waste state or disposal of final residues during the
environmental impacts have been calculated over the calendar construction process stage.
year 2022.
The end-of-life stage is a mandatory information module and it
The EPD is studied for a common product thickness of 80mm. covers:
Multiplication factors are included to calculate impacts for other - C1 de-construction, demolition;
product thicknesses within the range of 50 to 160 mm. - C2 transport to waste processing;
- C3 waste processing for reuse, recovery and/or recycling;
System boundary - C4 disposal (not applicable for this EPD) including provision
Type of EPD: according to EN 15804: cradle to gate with and all transport, provision of all materials, products and related
options, modules C1–C4, and module D (A1–A3, C, D and energy and water use.
additional modules: A4,A5).
Environmental burden of the incineration (R1 > 60%) of the
2 Environmental Product Declaration - Kingspan Insulation BV - Kooltherm® K15 C
product at the end-of-life stage are assigned to the product energy from energy substitution are declared in module D.
system (C3); resulting potential credits for thermal and electrical
Factors for different thicknesses
The LCA results for the insulation material declared in this EPD Geographic Representativeness
refer to a product with a thickness of 80 mm. To enable the user Land or region, in which the declared product system is
of the EPD to calculate the results for different thicknesses the manufactured, used or handled at the end of the product´s
factors in the following table can be used for the calculation. lifespan: Europe
The LCA results in chapter 5 have to be multiplied by these
factors. The scaling factors are applicable for the complete
Comparability
product, where the facings are for all product thicknesses
Basically, a comparison or an evaluation of EPD data is only
equal, and the foam inputs are scaling upwards and
possible if all the data sets to be compared were created
downwards with other product thicknesses.
according to EN 15804 and the building context, respectively
the product-specific characteristics of performance, are taken
Background data from GaBi ts Version 10 is used with GaBi
into account.
data sets CUP2022.1
LCA: Scenarios and additional technical information
Installation into the building (A5)
Characteristic product properties of biogenic carbon
The total mass of biogenic carbon containing materials is less Name ValueUnit
than 5 % of the total mass of the product and accompanying Output substances following waste treatment on
0.06 kg
packaging. site
Technical information
The recycling of the packaging is considered in A5.
The following technical information is a basis for the declared
modules or can be used for developing specific scenarios in the
context of a building assessment. End of life (C1-C4)
The assumptions for C1 are: diesel driven excavator (100 kW;
Manufacturing (A3) 0.02 litre fuel per ton excavated material). The assumptions for
Within A1-A3 the following packaging of the final product is C2 are: Truck Euro 6, diesel driven, 26-28 t gross weight,
included: assumed distance 50 km.
Polyethylene cover and wrap: 0,05 kg/m² Name Value Unit
Others (mainly Expanded Polystyrene skid): 0,01 kg/m²
Collected as mixed construction waste 3.035 kg
Energy recovery 3.035 kg
Transport to the building site (A4)
R1-value of waste incineration plant >60 %
Name Value Unit
Litres of fuel 0.0103 l/100km
Reuse, recovery and/or recycling potentials (D), relevant
Transport distance 100 km scenario information
Grammage of products transported 3,035 kg/m2 Waste incineration with energy recuperation is assumed as
end-of-life scenario.
3 Environmental Product Declaration - Kingspan Insulation BV - Kooltherm® K15 C
LCA: Results
DESCRIPTION OF THE SYSTEM BOUNDARY (X = INCLUDED IN LCA; ND = MODULE OR INDICATOR NOT DECLARED; MNR =
MODULE NOT RELEVANT)
Benefits and
Construction loads beyond
Product stage Use stage End of life stage
process stage the system
boundaries
la ire ta m w a Ry lp p u s tro p s n a rT g n iru tc a fu n a M e h t m o rf tro p s n a rTe tis e h t o t e ta g y lb m e s s A e s U e c n a n e tn ia M ria p e R tn e m e c a lp e R tn e m h s ib ru fe R y g re n e la n o ita re p Oe s u re ta w la n o ita re p Oe s u n o itc u rts n o c -e Dn o itilo m e d tro p s n a rT g n is s e c o rp e ts a W la s o p s iD -e s u e R-y re v o c e R-g n ilc y c e Rla itn e to p
A1 A2 A3 A4 A5 B1 B2 B3 B4 B5 B6 B7 C1 C2 C3 C4 D
X X X X X MND MND MNR MNR MNR MND MND X X X X X
RESULTS OF THE LCA - ENVIRONMENTAL IMPACT according to EN 15804+A2: 1 m2 80 mm thickness
Parameter Unit A1-A3 A4 A5 C1 C2 C3 C4 D
GWP-total kg CO 2 eq 6.67E+00 2.56E-02 1.5E-01 1.95E-03 1.28E-02 6.43E+00 0 -3.47E+00
GWP-fossil kg CO 2 eq 6.64E+00 2.55E-02 1.5E-01 1.95E-03 1.27E-02 6.43E+00 0 -3.45E+00
GWP-biogenic kg CO 2 eq -4.14E-02 -3.52E-05 8.17E-06 2.61E-06 -1.76E-05 4.37E-04 0 -1.53E-02
GWP-luluc kg CO 2 eq 6.77E-02 1.42E-04 1.77E-06 2.4E-08 7.11E-05 1.14E-05 0 -4.45E-04
ODP kg CFC11 eq 1.18E-08 1.53E-15 2.66E-14 1.2E-16 7.64E-16 4.71E-13 0 -1.77E-11
AP mol H+ eq 1.85E-02 2.63E-05 1.86E-05 9.05E-06 1.31E-05 3.79E-03 0 -8.07E-03
EP-freshwater kg P eq 2.12E-05 7.61E-08 6.73E-09 3.93E-10 3.81E-08 1.27E-07 0 -3.83E-06
EP-marine kg N eq 4.33E-03 8.59E-06 5E-06 4.31E-06 4.3E-06 1.84E-03 0 -1.45E-03
EP-terrestrial mol N eq 4.42E-02 1.02E-04 8.48E-05 4.72E-05 5.12E-05 2.11E-02 0 -1.57E-02
kg NMVOC
POCP 2.09E-02 2.31E-05 1.44E-05 1.22E-05 1.16E-05 4.72E-03 0 -4.26E-03
eq
ADPE kg Sb eq 1.75E+02 3.41E-01 5.52E-02 2.64E-02 1.7E-01 1.66E+00 0 -5.45E+01
ADPF MJ 5.86E-06 2.13E-09 6.5E-10 7.97E-11 1.07E-09 1.3E-08 0 -4.45E-07
m3 world eq
WDP 1.13E+00 2.29E-04 1.42E-02 3.62E-06 1.14E-04 6.34E-01 0 -4.18E-01
deprived
GWP = Global warming potential; ODP = Depletion potential of the stratospheric ozone layer; AP = Acidification potential of land and water; EP =
Eutrophication potential; POCP = Formation potential of tropospheric ozone photochemical oxidants; ADPE = Abiotic depletion potential for non-fossil
resources; ADPF = Abiotic depletion potential for fossil resources; WDP = Water (user) deprivation potential)
RESULTS OF THE LCA - INDICATORS TO DESCRIBE RESOURCE USE according to EN 15804+A2: 1 m2 80 mm thickness
Parameter Unit A1-A3 A4 A5 C1 C2 C3 C4 D
PERE MJ 2.33E+01 1.94E-02 1.42E-02 9.96E-05 9.69E-03 2.89E-01 0 -1.75E+01
PERM MJ 0 0 0 0 0 0 0 0
PERT MJ 2.33E+01 1.94E-02 1.42E-02 9.96E-05 9.69E-03 2.89E-01 0 -1.75E+01
PENRE MJ 9.02E+01 3.42E-01 2.6E+00 2.64E-02 1.71E-01 8.45E+01 0 -5.45E+01
PENRM MJ 8.54E+01 0 -2.55E+00 0 0 -8.29E+01 0 0
PENRT MJ 1.76E+02 3.42E-01 5.53E-02 2.64E-02 1.71E-01 1.66E+00 0 -5.45E+01
SM kg 0 0 0 0 0 0 0 0
RSF MJ 0 0 0 0 0 0 0 0
NRSF MJ 0 0 0 0 0 0 0 0
FW m3 5.76E-02 2.19E-05 3.37E-04 1.5E-07 1.1E-05 1.49E-02 0 -2.58E-02
PERE = Use of renewable primary energy excluding renewable primary energy resources used as raw materials; PERM = Use of renewable primary
energy resources used as raw materials; PERT = Total use of renewable primary energy resources; PENRE = Use of non-renewable primary energy
excluding non-renewable primary energy resources used as raw materials; PENRM = Use of non-renewable primary energy resources used as raw
materials; PENRT = Total use of non-renewable primary energy resources; SM = Use of secondary material; RSF = Use of renewable secondary fuels;
NRSF = Use of non-renewable secondary fuels; FW = Use of net fresh water
RESULTS OF THE LCA – WASTE CATEGORIES AND OUTPUT FLOWS according to EN 15804+A2:
1 m2 80 mm thickness
Parameter Unit A1-A3 A4 A5 C1 C2 C3 C4 D
HWD kg 7.95E-05 1.64E-12 4.6E-12 8.72E-14 8.18E-13 2.29E-10 0 -4.29E-09
NHWD kg 4.29E-01 4.89E-05 1.34E-02 2.47E-06 2.45E-05 3.24E-02 0 -2.94E-01
RWD kg 3.84E-03 4.21E-07 2.3E-06 2.9E-08 2.1E-07 6.85E-05 0 -4.11E-03
CRU kg 0 0 0 0 0 0 0 0
MFR kg 0 0 0 0 0 1.27E-01 0 0
MER kg 0 0 5.99E-02 0 0 2.91E+00 0 0
EEE MJ 0 0 2.72E-01 0 0 1.11E+01 0 0
EET MJ 0 0 4.86E-01 0 0 1.99E+01 0 0
HWD = Hazardous waste disposed; NHWD = Non-hazardous waste disposed; RWD = Radioactive waste disposed; CRU = Components for re-use;
MFR = Materials for recycling; MER = Materials for energy recovery; EEE = Exported electrical energy; EET = Exported thermal energy
4 Environmental Product Declaration - Kingspan Insulation BV - Kooltherm® K15 C
RESULTS OF THE LCA – additional impact categories according to EN 15804+A2-optional:
1 m2 80 mm thickness
Parameter Unit A1-A3 A4 A5 C1 C2 C3 C4 D
Disease
PM 1.97E-07 1.52E-10 2.27E-10 1.03E-10 7.58E-11 1.05E-08 0 -7.7E-08
incidence
IR kBq U235 eq 5.97E-01 6.16E-05 3.16E-04 4.21E-06 3.08E-05 1.1E-02 0 -7.26E-01
ETP-fw CTUe 7.06E+01 2.37E-01 3.95E-02 1.84E-02 1.18E-01 5.66E-01 0 -1.37E+01
HTP-c CTUh 2.91E-09 4.77E-12 2.22E-12 3.39E-13 2.38E-12 4.28E-11 0 -9.98E-10
HTP-nc CTUh 1.02E-07 2.47E-10 2.24E-10 1.72E-11 1.24E-10 1.55E-09 0 -2.82E-08
SQP SQP 1.49E+01 1.17E-01 1.41E-02 7.27E-05 5.86E-02 3.47E-01 0 -8.03E+00
PM = Potential incidence of disease due to PM emissions; IR = Potential Human exposure efficiency relative to U235; ETP-fw = Potential comparative
Toxic Unit for ecosystems; HTP-c = Potential comparative Toxic Unit for humans (cancerogenic); HTP-nc = Potential comparative Toxic Unit for humans
(not cancerogenic); SQP = Potential soil quality index
Disclaimer 1 – for the indicator “Potential Human exposure efficiency relative to U235”. This impact category deals mainly with the
eventual impact of low-dose ionizing radiation on human health of the nuclear fuel cycle. It does not consider effects due to possible
nuclear accidents, occupational exposure or radioactive waste disposal in underground facilities. Potential ionizing radiation from the
soil, radon and from some construction materials is also not measured by this indicator.
Disclaimer 2 – for the indicators “abiotic depletion potential for non-fossil resources”, “abiotic depletion potential for fossil resources”,
“water (user) deprivation potential, deprivation-weighted water consumption”, “potential comparative toxic unit for ecosystems”,
“potential comparative toxic unit for humans – cancerogenic”, “Potential comparative toxic unit for humans - not cancerogenic”,
“potential soil quality index”. The results of this environmental impact indicator shall be used with care as the uncertainties on these
results are high as there is limited experience with the indicator.
This EPD was created using a software tool.
References
EN 13166
EN 13166:2012+A2:2016: Thermal insulation products for ISO 14025
buildings. Factory made phenolic foam (PF) products. EN ISO 14025:2011-10 - Environmental labels and declarations
Specification — Type III environmental declarations — Principles and
procedures
EN 15804
EN 15804:2012+A2:2019+AC:2021, Sustainability of LCA-tool
construction works - Kingspan LCA tool, version 1.2. IBU-KSI-202001-LT1-EN.
Environmental product declarations - Core rules for the product Developed by Sphera Solutions GmbH (formely Thinkstep
category of construction products GmbH)
BPR PCR Version 1.7, Part A
Regulation (EU) No 528/2012 of the European Parliament and Institut Bauen und Umwelt e.V., Berlin (pub.): Product Category
of the Council of 22 May 2012 concerning the making available Rules for Building-Related Products andservices, Part A:
on the market and use of biocidal products Calculation Rules for the Life Cycle Assessment and
Requirements on the Project Report according to EN
15804+A2:2019 November 2021
CPR
Regulation (EU) No. 305/2011 of the European Parliament and
of the Council of 9 March 2011 laying down harmonised PCR, Part B
condition for the marketing of construction products and Institut Bauen und Umwelt e.V., Berlin (pub.): Product Category
repealing Council Directive 89/106/EC Rules for Construction Products from the range of
Environmental Product Declarations of Institut Bauen und
Umwelt (IBU), Part B: Requirements on the EPD for insulating
GaBi ts materials made of foam plastics. June 2023
thinkstep AG: Leinfelden-Echterdingen GaBi Software- System
and Database for Life Cycle Engineering 1992-2019
REACH
Regulation (EC) No 1907/2006 of the European Parliament and
IBU 2021 of the Council on the Registration, Evaluation, Authorisation
Institut Bauen und Umwelt e.V.: General Instructions for the and Restriction of Chemicals (REACH)
EPD programme of Institut Bauen und Umwelte.V., Version 2.0, https://echa.europa.eu/candidate-list-table; accessed 17th of
Berlin: Institut Bauen und Umwelte.V., 2021. www.ibu-epd.com January 2023, 233 substances listed.
5 Environmental Product Declaration - Kingspan Insulation BV - Kooltherm® K15 C
Publisher
Institut Bauen und Umwelt e.V. +49 (0)30 3087748- 0
Hegelplatz 1 info@ibu-epd.com
10117 Berlin www.ibu-epd.com
Germany
Programme holder
Institut Bauen und Umwelt e.V. +49 (0)30 3087748- 0
Hegelplatz 1 info@ibu-epd.com
10117 Berlin www.ibu-epd.com
Germany
Author of the Life Cycle Assessment
Kingspan Insulation B.V. +31 (0) 543 543 210
Lingewei 8 info@kingspaninsulation.nl
4004LL Tiel www.kingspan.com
Netherlands
Owner of the Declaration
Kingspan Insulation B.V. +31 (0) 543 543 210
Lingewei 8 info@kingspaninsulation.nl
4004LL Tiel www.kingspan.com
Netherlands
6 Environmental Product Declaration - Kingspan Insulation BV - Kooltherm® K15 C
