ENVIRONMENTAL PRODUCT DECLARATION
as per ISO 14025 and EN 15804+A2
Owner of the Declaration Kronospan Luxembourg S.A.
Publisher Institut Bauen und Umwelt e.V. (IBU)
Programme holder Institut Bauen und Umwelt e.V. (IBU)
Declaration number EPD-KRO-20230158-CBA1-EN
Issue date 11.07.2023
Valid to 10.07.2028
Kronospan Laminate Flooring
Kronospan Luxembourg S.A.
www.ibu-epd.com | https://epd-online.com
General Information
Kronospan Luxembourg S.A. Kronospan Laminate Flooring
Programme holder Owner of the declaration
IBU – Institut Bauen und Umwelt e.V. Kronospan Luxembourg S.A.
Hegelplatz 1 Rue GadderScheier 1
10117 Berlin 4984 Soleuvre
Germany Luxembourg
Declaration number Declared product / declared unit
EPD-KRO-20230158-CBA1-EN 1m2 Kronospan flooring products made of HDF
This declaration is based on the product category rules: Scope:
Floor coverings, 01.08.2021 This document applies to Kronospan flooring products made of HDF, which
(PCR checked and approved by the SVR) is composed of wood shavings, mixed with a resin (melamine urea
formaldehyde – MUF).
The declared unit weight is 6.91 kg/m2. LCA data were compiled using
Issue date foreground data collected based on billing documents and material
balances for the period between October 2020 and March 2022.
11.07.2023
The declaration holder is responsible for the underlying data and its
verification.
The owner of the declaration shall be liable for the underlying information
Valid to
and evidence; the IBU shall not be liable with respect to manufacturer
10.07.2028 information, life cycle assessment data and evidences.
The EPD was created according to the specifications of EN 15804+A2. In
the following, the standard will be simplified as EN 15804.
Verification
The standard EN 15804 serves as the core PCR
Independent verification of the declaration and data according to ISO
14025:2011
internally X externally
Dipl.-Ing. Hans Peters
(Chairman of Institut Bauen und Umwelt e.V.)
Florian Pronold Mr Olivier Muller,
(Managing Director Institut Bauen und Umwelt e.V.) (Independent verifier)
1 Environmental Product Declaration - Kronospan Luxembourg S.A. - Kronospan Laminate Flooring
Product
Product description/Product definition Technical Data
Direct pressure laminate (DPL) floor coverings described in this
Constructional data
EPD are produced by member companies of EPLF®. The floor
Name Value Unit
coverings meet the requirements of EN 13329.
DPL floorings consist of a number of layers. On the top side Grammage 6910 g/m2
there is a decor with a transparent, wear-resistant contact Abrasion Class AC3-AC5 -
surface; in the middle there is a core layer made of high-density
Product Form panel -
wood fibers (HDF) and on the back side there is a stabilizing
Thickness of the element 6 - 12 mm
layer to guarantee floor stability.
Length of the surface layer 300 - 2500 mm
The decorative paper of a DPL floor covering can be printed Width of the surface layer 70 - 400 mm
with any design and gives the floor its individual appearance. Length and width of squared elements 250 - 700 mm
For the placing on the market of the product in the European Density 800 - 1200 kg/m3
Union/European Free Trade Association (EU/EFTA) (with the
exception of Switzerland) Regulation (EU) No. 305/2011 (CPR) Performance data of the product in accordance with the
applies. The product needs a declaration of performance taking declaration of performance with respect to its essential
into consideration EN 13329:2016 + A2:2021 - Laminate Floor characteristics according to EN 13329 : 2016 + A2:2021.
coverings - Elements with a surface layer based on
Base materials/Ancillary materials
aminoplastic thermosetting resins - Specifications,
The flooring product is made of high-density fibreboard (HDF)
Requirements and test methods - and the CE-marking.
(94% of the product weight) and of melamine impregnated
Application paper (6% of product weight).
The laminate floor covering described in this EPD is intended to
be used within a building and meets the requirements of the This product contains substances listed in the candidate list
use classes: 21-23, 31-33 according to EN 13329:2016 + (date: 28/02/2023) exceeding 0.1 percentage by mass: NO.
A2:2021 - Laminate Floor coverings - Elements with a surface
Reference service life
layer based on aminoplastic thermosetting resins -
The service life of resilient floor coverings depends on the
Specifications, Requirements and test methods, EN ISO
correct installation taking into account the declared use
10874:2012 / A1:2020- Resilient, textile and laminate floor
classification and the adherence to cleaning and maintenance
coverings - Classification .
instructions.
For the application and use the respective national provisions
A minimum service life of 20 years can be assumed /BNB/,
apply.
technical service life can be considerably longer.
LCA: Calculation rules
Declared Unit The ecoinvent database version 3.8 was used to model
This declaration applies to 1 m2 of Kronospan flooring products, background data. The average dataset based on European
with a declared unit weight of 6.91 kg/m2. data is used to model the glue production (no specific supplier
data used).
Declared unit and mass reference
Name Value Unit System boundary
Declared unit 1 m2 Type of EPD: Cradle-to-grave (with options)
Grammage 6.91 kg/m2 The system boundaries of the EPD follow the modular
construction system as described by EN 15804.
Layer thickness 0.007 m
Foreground data for the production processes (A1-A3) were The LCA considers the following modules:
collected from the Kronospan production site (Sanem, - A1-A3: Manufacturing of pre-products, packaging, ancillary
Luxembourg) and are and representative for the period of materials, transport to the factory and production, with the
October 2020 to March 2022. The manufacturing data are associated energy supply and waste handling
specific to the technologies used in the plant and representative - A4: Transport to the construction site
of the local geographical context. Market share data specific to - A5: Installation into the building including disposal of
each product category from the year 2021 were used to model packaging
the transport to building site (module A4). - B2: Maintenance, including the flooring cleaning
- C1: Deconstruction
For the further life cycle stages (modules A5 to D), generic - C2: Transport to disposal sites
inventory data are used. These processes are not specific to - C3: Final product waste disposal for reuse, recycling and
Kronospan products and reference data or statistics were energy recovery
applied. The inputs of outputs of these processes were mainly - C4: Waste disposal, namely incineration and landfill
based on the COFIDAB report prepared by FCBA (2012) and - D: Potential for reuse, recovery and/or recycling including
associated French EPD ('FDES') published by FCBA, as well benefits for product incineration from module C4
as EPDs of similar products for cleaning data (PURLINE, 2019;
Geographic Representativeness
ERFMI, 2019). The shares between various disposal routes for
packaging waste (module A5) were based on European Land or region, in which the declared product system is
statistics for the year 2019. manufactured, used or handled at the end of the product´s
2 Environmental Product Declaration - Kronospan Luxembourg S.A. - Kronospan Laminate Flooring
lifespan: Luxembourg Basically, a comparison or an evaluation of EPD data is only
possible if all the data sets to be compared were created
according to EN 15804 and the building context, respectively
Comparability
the product-specific characteristics of performance, are taken
into account.
LCA: Scenarios and additional technical information
Maintenance (B2)
Characteristic product properties of biogenic carbon
Name Value Unit
Information on describing the biogenic Carbon Content at
Water consumption (yearly value) 0.0145 m3
factory gate
Auxiliary (detergent) (yearly value) 0.045 kg
Name ValueUnit
Electricity consumption (yearly value) 0.271 kWh
kg
Biogenic carbon content in product 2.52
C
End of Life (C1-C4)
Biogenic carbon content in accompanying kg
0.354 Name Value Unit
packaging C
Collected as mixed construction waste 6.91 kg
Energy recovery 5.73 kg
Landfilling 1.17 kg
Transport to the construction site (A4)
Name Value Unit Reuse, recovery and/or recycling potentials (D), relevant
scenario information
Transport distance 864 km
Name Value Unit
Gross density of products transported 7.29 kg/m2
Avoided energy from incineration 80.2 MJ
Installation in the building (A5)
Name Value Unit
Material loss 0.628 kg
Product loss to incineration 83 %
Product loss to landfill 17 %
Packaging waste 0.328 kg
3 Environmental Product Declaration - Kronospan Luxembourg S.A. - Kronospan Laminate Flooring
LCA: Results
The results displayed below apply to 1 m2 of Kronospan flooring products made of HDF, with a declared unit weight of 6.91 kg/m2.
DESCRIPTION OF THE SYSTEM BOUNDARY (X = INCLUDED IN LCA; ND = MODULE OR INDICATOR NOT DECLARED; MNR =
MODULE NOT RELEVANT)
Benefits and
Construction loads beyond
Product stage Use stage End-of-life stage
process stage the system
boundaries
la ire ta m w a Ry lp p u s tro p s n a rT g n iru tc a fu n a M e h t m o rf tro p s n a rTe tis e h t o t e ta g y lb m e s s A e s U e c n a n e tn ia M ria p e R tn e m e c a lp e R tn e m h s ib ru fe R y g re n e la n o ita re p Oe s u re ta w la n o ita re p Oe s u n o itc u rts n o c -e Dn o itilo m e d tro p s n a rT g n is s e c o rp e ts a W la s o p s iD -e s u e R-y re v o c e R-g n ilc y c e Rla itn e to p
A1 A2 A3 A4 A5 B1 B2 B3 B4 B5 B6 B7 C1 C2 C3 C4 D
X X X X X MND X MNR MNR MNR MND MND X X X X X
RESULTS OF THE LCA - ENVIRONMENTAL IMPACT according to EN 15804+A2: 1 m2 Kronospan flooring products
Parameter Unit A1-A3 A4 A5 B2 C1 C2 C3 C4 D
GWP-total kg CO 2 eq -5.84E+00 6.17E-01 1.07E+00 4.07E-01 0 5.75E-02 0 1.09E+01 -2.4E+00
GWP-fossil kg CO 2 eq 6.06E+00 6.16E-01 2.62E-02 2.06E-01 0 5.74E-02 0 6.24E-02 -2.4E+00
GWP-biogenic kg CO 2 eq -1.19E+01 6.27E-04 1.04E+00 6.24E-02 0 5.16E-05 0 1.09E+01 -4.45E-04
GWP-luluc kg CO 2 eq 2.34E-02 2.21E-04 5.71E-06 1.39E-01 0 2.25E-05 0 2.11E-05 -7.51E-05
ODP kg CFC11 eq 6.63E-07 1.47E-07 3.16E-09 1.95E-08 0 1.33E-08 0 9.76E-09 -3.36E-07
AP mol H+ eq 3.63E-02 2.57E-03 2.22E-04 1.77E-03 0 2.33E-04 0 1.86E-03 -3.09E-03
EP-freshwater kg P eq 3.14E-04 4.21E-06 1.79E-07 7.65E-04 0 4.02E-07 0 1.06E-06 -2.19E-06
EP-marine kg N eq 5.77E-03 7.77E-04 1.23E-04 1.51E-03 0 6.94E-05 0 8.98E-04 -1.12E-03
EP-terrestrial mol N eq 8.19E-02 8.58E-03 1.1E-03 4.86E-03 0 7.67E-04 0 9.9E-03 -1.23E-02
kg NMVOC
POCP 2.64E-02 2.76E-03 3.04E-04 9.13E-04 0 2.35E-04 0 2.62E-03 -4.21E-03
eq
ADPE kg Sb eq 7.12E-05 1.41E-06 5.51E-08 2.97E-06 0 2E-07 0 2.24E-07 -1.42E-06
ADPF MJ 1E+02 9.6E+00 2.19E-01 3.34E+00 0 8.68E-01 0 8.02E-01 -3.35E+01
m3 world eq
WDP 7.57E+00 3.3E-02 2.44E-03 5.56E-01 0 2.6E-03 0 1.8E-02 -1.37E-02
deprived
GWP = Global warming potential; ODP = Depletion potential of the stratospheric ozone layer; AP = Acidification potential of land and water; EP =
Eutrophication potential; POCP = Formation potential of tropospheric ozone photochemical oxidants; ADPE = Abiotic depletion potential for non-fossil
resources; ADPF = Abiotic depletion potential for fossil resources; WDP = Water (user) deprivation potential)
RESULTS OF THE LCA - INDICATORS TO DESCRIBE RESOURCE USE according to EN 15804+A2: 1 m2 Kronospan flooring
products
Parameter Unit A1-A3 A4 A5 B2 C1 C2 C3 C4 D
PERE MJ 2.51E+00 1.22E-01 6.88E-03 4.6E+00 0 1.22E-02 0 8.02E+01 0
PERM MJ 1.88E+02 0 0 0 0 0 0 -8.02E+01 0
PERT MJ 1.91E+02 1.22E-01 6.88E-03 4.6E+00 0 1.22E-02 0 0 0
PENRE MJ 1.08E+02 1.02E+01 2.33E-01 3.7E+00 0 9.21E-01 0 8.62E-01 -3.72E+01
PENRM MJ 0 0 0 0 0 0 0 0 0
PENRT MJ 1.08E+02 1.02E+01 2.33E-01 3.7E+00 0 9.21E-01 0 8.62E-01 -3.72E+01
SM kg 0 0 0 0 0 0 0 0 0
RSF MJ 5.6E+01 0 0 0 0 0 0 0 8.02E+01
NRSF MJ 0 0 0 0 0 0 0 0 0
FW m3 2.7E-01 4.77E-03 4.61E-04 5.61E-02 0 5.35E-04 0 3.54E-03 -1.9E-03
PERE = Use of renewable primary energy excluding renewable primary energy resources used as raw materials; PERM = Use of renewable primary
energy resources used as raw materials; PERT = Total use of renewable primary energy resources; PENRE = Use of non-renewable primary energy
excluding non-renewable primary energy resources used as raw materials; PENRM = Use of non-renewable primary energy resources used as raw
materials; PENRT = Total use of non-renewable primary energy resources; SM = Use of secondary material; RSF = Use of renewable secondary fuels;
NRSF = Use of non-renewable secondary fuels; FW = Use of net fresh water
RESULTS OF THE LCA – WASTE CATEGORIES AND OUTPUT FLOWS according to EN 15804+A2:
1 m2 Kronospan flooring products
Parameter Unit A1-A3 A4 A5 B2 C1 C2 C3 C4 D
HWD kg 1.52E-04 2.32E-05 5.22E-07 1.12E-04 0 2.27E-06 0 1.87E-06 -4.49E-05
NHWD kg 9.42E-01 8.98E-01 2.14E-01 5.67E-02 0 4.46E-02 0 1.21E+00 -1.83E-02
RWD kg 1.9E-04 6.5E-05 1.23E-06 2.07E-05 0 5.87E-06 0 2.96E-06 -3.8E-06
CRU kg 0 0 0 0 0 0 0 0 0
MFR kg 0 0 0 0 0 0 0 0 0
MER kg 0 0 5.53E-01 0 0 0 0 5.73E+00 0
EEE MJ 0 0 0 0 0 0 0 0 0
EET MJ 0 0 1.28E+01 0 0 0 0 8.02E+01 0
4 Environmental Product Declaration - Kronospan Luxembourg S.A. - Kronospan Laminate Flooring
HWD = Hazardous waste disposed; NHWD = Non-hazardous waste disposed; RWD = Radioactive waste disposed; CRU = Components for re-use;
MFR = Materials for recycling; MER = Materials for energy recovery; EEE = Exported electrical energy; EET = Exported thermal energy
RESULTS OF THE LCA – additional impact categories according to EN 15804+A2-optional:
1 m2 Kronospan flooring products
Parameter Unit A1-A3 A4 A5 B2 C1 C2 C3 C4 D
Disease
PM 8.36E-07 7.23E-08 2.39E-09 1.89E-08 0 4.94E-09 0 1.62E-08 -9.6E-09
incidence
IR kBq U235 eq 1.55E-01 4.16E-02 8.54E-04 2.44E-02 0 3.77E-03 0 2.34E-03 -3.14E-03
ETP-fw CTUe 1.45E+02 7.5E+00 3.62E-01 2.11E+01 0 6.77E-01 0 1.44E+00 -2.7E+00
HTP-c CTUh 1.66E-08 2.07E-10 1.71E-10 3.77E-10 0 2.19E-11 0 1.71E-09 -1.44E-10
HTP-nc CTUh 1.15E-07 8.21E-09 6.96E-10 8.41E-09 0 7.1E-10 0 5.21E-09 -7.56E-09
SQP SQP 4.41E+02 1.1E+01 2.16E-01 9.2E+00 0 5.96E-01 0 8.47E-01 -6.55E-01
PM = Potential incidence of disease due to PM emissions; IR = Potential Human exposure efficiency relative to U235; ETP-fw = Potential comparative
Toxic Unit for ecosystems; HTP-c = Potential comparative Toxic Unit for humans (cancerogenic); HTP-nc = Potential comparative Toxic Unit for humans
(not cancerogenic); SQP = Potential soil quality index
Disclaimer 1 – for the indicator “Potential Human exposure efficiency relative to U235”. This impact category deals mainly with the
eventual impact of low-dose ionizing radiation on human health of the nuclear fuel cycle. It does not consider effects due to possible
nuclear accidents, occupational exposure or radioactive waste disposal in underground facilities. Potential ionizing radiation from the
soil, radon and from some construction materials is also not measured by this indicator.
Disclaimer 2 – for the indicators “abiotic depletion potential for non-fossil resources”, “abiotic depletion potential for fossil resources”,
“water (user) deprivation potential, deprivation-weighted water consumption”, “potential comparative toxic unit for ecosystems”,
“potential comparative toxic unit for humans – cancerogenic”, “Potential comparative toxic unit for humans - not cancerogenic”,
“potential soil quality index”. The results of this environmental impact indicator shall be used with care as the uncertainties on these
results are high as there is limited experience with the indicator.
References
Standards Declaration number EPD-ERF-20180185-CCI1-EN
ISO 14025 FCBA (2012)
ISO 14025:2007-10, Umweltkennzeichnungen und - Rapport d'étude Volet 2 – Prise en compte de la fin de vie des
deklarationen - Typ III produits bois. Convention DHUP/CSTB 2009 Action 33 – Sous
Umweltdeklarationen - Grundsätze und Verfahren (ISO action 5. ACV & Déclarations environnementales pour des
14025:2006) produits et composants de la construction bois.
EN 13329:2016 + A2:2021 FCBA (2019)
Laminate Floor coverings - Elements with a surface layer based Fiche de déclaration environmentale et sanitaire (FDES) –
on aminoplastic thermosetting resins - Specifications, Panneaux de lamelles de bois minces orientées OSB (oriented
Requirements and test methods strand board) de type 3 (panneaux travaillants utilisés en milieu
humide) bruts. Epaisseur déclarée : 18 mm. FDES collective 2-
EN ISO 10874:2012 / A1:2020 90 :2018.
Resilient, textile and laminate floor coverings — Classification .
FCBA (2022a)
EN 15804 + A2 (2019) Fiche de déclaration environmentale et sanitaire (FDES) –
Sustainability of construction works – Environmental product Panneaux de lamelles de bois minces orientées OSB (oriented
declarations – Core rules for the product category of strand board) de type 3 (panneaux travaillants utilisés en milieu
construction products. EN 15804:2012+A2:2019 humide) bruts. Epaisseur déclarée : 12 mm. FDES collective
132289692502022.
Further References
FCBA (2022b)
PCR 2021, Part A Fiche de déclaration environmentale et sanitaire (FDES) –
PCR Guidance-Texts for Building-Related Products and Panneaux de fibres MDF (medium-density fibrebord) utilisés en
Services: Calculation Rules for the Life Cycle Assessment and milieu humide bruts. Epaisseur déclarée : 18 mm. FDES
Requirements on the Project Report according to EN collective 182289782502022.
15804+A2:2019
FCBA (2022c)
PCR 2023, Part B Fiche de déclaration environmentale et sanitaire (FDES) –
PCR Guidance-Texts for Building-Related Products and Panneaux de fibres MDF (medium-density fibrebord) utilisés en
Services: Requirements on the EPD for Floor coverings milieu humide bruts. Epaisseur déclarée : 19 mm. FDES
collective 341289752502022.
BNB
Bewertungssystem Nachhaltiges Bauen PURLINE (2019)
https://www.nachhaltigesbauen.de/austausch/nutzungsdauern- Environmental Product Declaration (EPD) – Resilient
von-bauteilen/ polyurethane floor covering as planks for clicking. Declaration
number EPD-WIN-20190006-CCA1-EN
ERFMI (2019)
Environmental Product Declaration (EPD) – Semi flexible LVT SimaPro software and ecoinvent database:2021
floating floor with mechanical locking according to ISO 10582. SimaPro software ecoinvent database, version 3.8, 2021
5 Environmental Product Declaration - Kronospan Luxembourg S.A. - Kronospan Laminate Flooring
6 Environmental Product Declaration - Kronospan Luxembourg S.A. - Kronospan Laminate Flooring
Publisher
Institut Bauen und Umwelt e.V. +49 (0)30 3087748- 0
Hegelplatz 1 info@ibu-epd.com
10117 Berlin www.ibu-epd.com
Germany
Programme holder
Institut Bauen und Umwelt e.V. +49 (0)30 3087748- 0
Hegelplatz 1 info@ibu-epd.com
10117 Berlin www.ibu-epd.com
Germany
Author of the Life Cycle Assessment
Luxembourg Institute of Science and Technology 00352-275888-1
(LIST) info@list.lu
Avenue des Hauts-Fourneaux 5 www.list.lu
4362 Esch/Alzette
Luxembourg
Owner of the Declaration
Kronospan Luxembourg S.A. +352590311214
Rue GadderScheier 1 j.guerlot@kronospan.lu
4984 Soleuvre www.kronospan.lu
Luxembourg
7 Environmental Product Declaration - Kronospan Luxembourg S.A. - Kronospan Laminate Flooring
