ENVIRONMENTAL PRODUCT DECLARATION
as per ISO 14025 and EN 15804+A2
Owner of the Declaration Kronospan Luxembourg S.A.
Publisher Institut Bauen und Umwelt e.V. (IBU)
Programme holder Institut Bauen und Umwelt e.V. (IBU)
Declaration number EPD-KRO-20230157-CBA1-EN
Issue date 11.07.2023
Valid to 10.07.2028
Oriented Strand Board (OSB)
Kronospan Luxembourg S.A.
www.ibu-epd.com | https://epd-online.com
General Information
Kronospan Luxembourg S.A. Oriented Strand Board (OSB)
Programme holder Owner of the declaration
IBU – Institut Bauen und Umwelt e.V. Kronospan Luxembourg S.A.
Hegelplatz 1 Rue GadderScheier 1
10117 Berlin 4984 Soleuvre
Germany Luxembourg
Declaration number Declared product / declared unit
EPD-KRO-20230157-CBA1-EN 1m3 Oriented Strand Board (OSB)
This declaration is based on the product category rules: Scope:
Wood-based panels, 01.08.2021 This document applies to Oriented Strand Board (OSB), which is a
(PCR checked and approved by the SVR) structural-use panel based on layered wood strands bonded with water-
resistant resin. The declared unit weight is 630 kg/m3. LCA data were
compiled using foreground data collected based on billing documents and
Issue date material balances for the period between October 2020 and March 2022.
The declaration holder is responsible for the underlying data and its
11.07.2023
verification.
The owner of the declaration shall be liable for the underlying information
and evidence; the IBU shall not be liable with respect to manufacturer
Valid to
information, life cycle assessment data and evidences.
10.07.2028
The EPD was created according to the specifications of EN 15804+A2. In
the following, the standard will be simplified as EN 15804.
Verification
The standard EN 15804 serves as the core PCR
Independent verification of the declaration and data according to ISO
14025:2011
internally X externally
Dipl.-Ing. Hans Peters
(Chairman of Institut Bauen und Umwelt e.V.)
Florian Pronold Mr Olivier Muller,
(Managing Director Institut Bauen und Umwelt e.V.) (Independent verifier)
1 Environmental Product Declaration - Kronospan Luxembourg S.A. - Oriented Strand Board (OSB)
Product
For more details on technical information, please see technical
Product description/Product definition brochure Kronobuild.
Oriented Strand Board (OSB) are wooden panels made from
oriented wood strands connected by resin, in range of Quality assurance according to EN 300 and EN
thickness 6-38 mm. OSB is developed and manufactured 13986:2004+A1:2015 - type OSB 3. Reaction to fire
entirely in compliance with the current demand of ecological classification acc. EN 13501-1: class D-s2,d0 for thicknesses 8-
living focused on organic materials. Selecting suitable wood 38 mm.
and binder, OSB meets high standards of not only
Constructional data
environmental buildings.
Name Value Unit
Product characteristics: 580 -
Gross density kg/m3
680
• High durability and resistance
• High load-bearing capacity Grammage 4.64 - kg/m2
• High performance material 25.84
• High stability Bending strength (longitudinal) acc. to EN
14 - 22 N/mm2
For the placing on the market of the product in the European 310
Union/European Free Trade Association (EU/EFTA) (with the Bending strength (transverse) acc. to EN 310 7 - 11 N/mm2
exception of Switzerland) Regulation (EU) No. 305/2011 (CPR)
E-module (longitudinal) acc. to EN 310 ≥ 3500 N/mm2
applies. The product needs a declaration of performance taking
into consideration EN 13986:2004 + A1:2015, Wood-based E-module (transverse) acc. to EN 310 ≥ 1400 N/mm2
panels for use in construction - Characteristics, evaluation of Material dampness at delivery acc. to EN 322 2 - 12 %
conformity and marking - and the CE-marking. For the 0.26 -
application and use the respective national provisions apply. Tensile strength rectangular acc. to EN 319 0.34 N/mm2
Thermal conductivity acc. to EN 13986 0.1 W/(mK)
Application
- Load-bearing cladding of exterior walls or roofs Formaldehyde emissions E1 acc. to EN 717- - μg/m3
- Structural floor decking 1 or E1 DE 2020 ChemVerbotsV (E05)
- Sub- floors and base boards for flooring systems Performance data of the product in accordance with the
- Internal non load-bearing cladding of walls and ceilings, declaration of performance with respect to its essential
partitions characteristics according to EN 13986:2004 + A1:2015.
- Attic conversions or extensions
- Framework for upholstered furniture Base materials/Ancillary materials
- Packaging The OSB3 panels are made of 84% of vigin wood, 12% of
- Warehouse management (racks, fences, etc.) recycled wood, 3% of polymeric isocyanate (pMDI), and 1,5%
of other additives.
Technical Data
This product contains substances listed in the candidate list
Performance data of the product are in accordance with its (date: 08.03.2023) exceeding 0.1 percentage by mass: no.
Declaration of performance (DoP) and with respect to the
Essential characteristics according to : Reference service life
The service life is assumed to be 100 years, as OSB is a
• EN 13986 + A1:2015 Wood-based panels for use in
structural element of a building.
construction - Characteristics, evaluation of conformity
and marking.
Since no use impacts are quantified (the products do not
• EN 300 - Oriented Strand Boards (OSB) - Definitions,
require energy, maintenance or other reparation process during
Classification and Specifications.
its use), this lifetime parameter does not influence the results.
LCA: Calculation rules
Declared Unit For the further life cycle stages (modules A5 to D), generic
This declaration applies to 1 m3 of Oriented Strand Board inventory data are used. These processes are not specific to
(OSB), with a declared unit weight of 630 kg/m3. Kronospan products and reference data or statistics were
Declared unit and mass reference applied. The inputs of outputs of these processes were mainly
based on the COFIDAB report prepared by FCBA (2012) and
Name Value Unit
associated French EPD ('FDES') published by FCBA. The
Declared unit 1 m3 shares between various disposal routes for packaging waste
Mass reference 630 kg/m3 (module A5) were based on European statistics for the year
Layer thickness 0.016 m 2019.
Foreground data for the production processes (A1-A3) were
The ecoinvent database version 3.8 was used to model
collected from the Kronospan production site (Sanem,
background data. The average dataset based on European
Luxembourg) and are and representative for the period of
data is used to model the glue production (no specific supplier
October 2020 to March 2022. The manufacturing data are
data used).
specific to the technologies used in the plant and representative
of the local geographical context. Market share data specific to System boundary
each product category from the year 2021 were used to model Type of EPD: Cradle-to-grave (with options) The system
the transport to building site (module A4). boundaries of the EPD follow the modular construction system
2 Environmental Product Declaration - Kronospan Luxembourg S.A. - Oriented Strand Board (OSB)
as described by EN 15804. - D: Potential for reuse, recovery and/or recycling including
benefits for product incineration from module C4
The LCA considers the following modules:
- A1-A3: Manufacturing of pre-products, packaging, ancillary Geographic Representativeness
materials, transport to the factory and production, with the Land or region, in which the declared product system is
associated energy supply and waste handling manufactured, used or handled at the end of the product´s
- A4: Transport to the construction site lifespan: Luxembourg
- A5: Installation into the building including disposal of
packaging
Comparability
- C1: Deconstruction (screws disposal and electricity from the
Basically, a comparison or an evaluation of EPD data is only
screwdriver)·
possible if all the data sets to be compared were created
- C2: Transport to disposal sites
according to EN 15804 and the building context, respectively
- C3: Final product waste disposal for reuse, recycling and
the product-specific characteristics of performance, are taken
energy recovery
into account.
- C4: Waste disposal, namely incineration and landfill
LCA: Scenarios and additional technical information
Name Value Unit
Characteristic product properties of biogenic carbon
Auxiliary (screw) 1.48 kg
The biogenic carbon content quantifies the amount of biogenic
Electricity consumption 0.062 kWh
carbon in a construction product leaving the factory gate, and it
shall be separately declared for the product and for any Material loss 50.4 kg
accompanying packaging. Product loss to recycling 57.5 %
If the total mass of biogenic carbon containing materials is less Product loss to incineration 25.5 %
than 5 % of the total mass of the product and accompanying
Product loss to landfill 17 %
packaging, the declaration of biogenic carbon content may be
Packaging waste 11.01 kg
omitted. The mass of packaging containing biogenic carbon
shall always be declared. The refence service life does not affect the results since no use
impacts are quantified.
Note: 1 kg of biogenic carbon is equivalent to 44/12 kg of CO2.
End of life (C1-C4)
Name Value Unit
Information on describing the biogenic Carbon Content at
Collected separately 425.5 kg
factory gate
Collected as mixed construction waste 204.8 kg
Name ValueUnit
Recycling 362.4 kg
kg
Biogenic carbon content in product 360.9 Energy recovery 160.7 kg
C
Landfilling 107.2 kg
Biogenic carbon content in accompanying kg
13.9
packaging C
Reuse, recovery and/or recycling potentials (D), relevant
scenario information
Name Value Unit
Transport to the building site (A4) Avoided virgin wood production 362 kg
Name Value Unit Avoided virgin wood transport 26.5 tkm
Transport distance (truck) 501 km Avoided drying energy 100 MJ
Gross density of products transported 640.5 kg/m3 Avoided energy from incineration 2249 MJ
Installation into the building (A5)
3 Environmental Product Declaration - Kronospan Luxembourg S.A. - Oriented Strand Board (OSB)
LCA: Results
The results displayed below apply to 1 m3 of Kronospan OSB3 panel, with a declared unit weight of 630 kg/m3.
DESCRIPTION OF THE SYSTEM BOUNDARY (X = INCLUDED IN LCA; ND = MODULE OR INDICATOR NOT DECLARED; MNR =
MODULE NOT RELEVANT)
Benefits and
Construction loads beyond
Product stage Use stage End-of-life stage
process stage the system
boundaries
la ire ta m w a Ry lp p u s tro p s n a rT g n iru tc a fu n a M e h t m o rf tro p s n a rTe tis e h t o t e ta g y lb m e s s A e s U e c n a n e tn ia M ria p e R tn e m e c a lp e R tn e m h s ib ru fe R y g re n e la n o ita re p Oe s u re ta w la n o ita re p Oe s u n o itc u rts n o c -e Dn o itilo m e d tro p s n a rT g n is s e c o rp e ts a W la s o p s iD -e s u e R-y re v o c e R-g n ilc y c e Rla itn e to p
A1 A2 A3 A4 A5 B1 B2 B3 B4 B5 B6 B7 C1 C2 C3 C4 D
X X X X X MND MND MNR MNR MNR MND MND X X X X X
RESULTS OF THE LCA - ENVIRONMENTAL IMPACT according to EN 15804+A2: 1 m3 Kronospan OSB3 panel
Parameter Unit A1-A3 A4 A5 C1 C2 C3 C4 D
GWP-total kg CO 2 eq -1.22E+03 3.16E+01 1.15E+02 2.53E-02 5.24E+00 9.01E+02 4.43E+02 6.62E+02
GWP-fossil kg CO 2 eq 2.18E+02 3.16E+01 3.9E+00 2.45E-02 5.24E+00 7.2E+00 1.77E+00 -9.95E+01
GWP-biogenic kg CO 2 eq -1.44E+03 3.21E-02 1.12E+02 7.69E-04 4.71E-03 8.94E+02 4.41E+02 7.63E+02
GWP-luluc kg CO 2 eq 1.92E+00 1.14E-02 2.66E-03 5.78E-05 2.06E-03 1.56E-02 5.43E-04 -1E+00
ODP kg CFC11 eq 4.98E-05 7.54E-06 3.2E-07 1.23E-09 1.21E-06 4.2E-07 4.36E-07 -1.52E-05
AP mol H+ eq 1.53E+00 1.32E-01 2.14E-02 1.39E-04 2.13E-02 5.77E-02 3.8E-02 -1.64E-01
EP-freshwater kg P eq 1.89E-02 2.16E-04 1.53E-04 2.61E-06 3.67E-05 7.05E-04 2.72E-05 -6.97E-03
EP-marine kg N eq 3.59E-01 3.98E-02 6.69E-03 1.77E-05 6.34E-03 1.44E-02 2.02E-02 -5.99E-02
EP-terrestrial mol N eq 3.46E+00 4.39E-01 6.81E-02 2.04E-04 7E-02 1.65E-01 1.95E-01 -6.05E-01
kg NMVOC
POCP 1.55E+00 1.41E-01 2.37E-02 5.62E-05 2.14E-02 4.4E-02 5.42E-02 -4.57E-01
eq
ADPE kg Sb eq 2.57E-03 7.24E-05 4.06E-05 2.27E-07 1.82E-05 6.33E-05 6.28E-06 -8.97E-05
ADPF MJ 4.45E+03 4.92E+02 4.34E+01 5.18E-01 7.92E+01 1.46E+02 3.32E+01 -1.44E+03
m3 world eq
WDP 1.34E+02 1.69E+00 8.21E-01 6.07E-03 2.37E-01 1.81E+00 4E-01 -4.84E+00
deprived
GWP = Global warming potential; ODP = Depletion potential of the stratospheric ozone layer; AP = Acidification potential of land and water; EP =
Eutrophication potential; POCP = Formation potential of tropospheric ozone photochemical oxidants; ADPE = Abiotic depletion potential for non-fossil
resources; ADPF = Abiotic depletion potential for fossil resources; WDP = Water (user) deprivation potential)
RESULTS OF THE LCA - INDICATORS TO DESCRIBE RESOURCE USE according to EN 15804+A2: 1 m3 Kronospan OSB3
panel
Parameter Unit A1-A3 A4 A5 C1 C2 C3 C4 D
PERE MJ 2.4E+02 6.26E+00 3.24E+00 1.04E-01 1.12E+00 8.82E+02 1.37E+03 0
PERM MJ 1.53E+04 0 0 0 0 -5.95E+03 -1.37E+03 0
PERT MJ 1.56E+04 6.26E+00 3.24E+00 1.04E-01 1.12E+00 -5.07E+03 0 0
PENRE MJ 4.78E+03 5.23E+02 4.59E+01 5.44E-01 8.41E+01 1.53E+02 3.54E+01 -1.59E+03
PENRM MJ 0 0 0 0 0 0 0 0
PENRT MJ 4.78E+03 5.23E+02 4.59E+01 5.44E-01 8.41E+01 1.53E+02 3.54E+01 -1.59E+03
SM kg 8.08E+01 0 0 0 0 0 0 3.62E+02
RSF MJ 9.76E+03 0 0 0 0 0 0 2.25E+03
NRSF MJ 0 0 0 0 0 0 0 0
FW m3 1.5E+01 2.44E-01 7.54E-02 8.67E-03 4.89E-02 2.34E+00 8.9E-02 -2.81E-01
PERE = Use of renewable primary energy excluding renewable primary energy resources used as raw materials; PERM = Use of renewable primary
energy resources used as raw materials; PERT = Total use of renewable primary energy resources; PENRE = Use of non-renewable primary energy
excluding non-renewable primary energy resources used as raw materials; PENRM = Use of non-renewable primary energy resources used as raw
materials; PENRT = Total use of non-renewable primary energy resources; SM = Use of secondary material; RSF = Use of renewable secondary fuels;
NRSF = Use of non-renewable secondary fuels; FW = Use of net fresh water
RESULTS OF THE LCA – WASTE CATEGORIES AND OUTPUT FLOWS according to EN 15804+A2:
1 m3 Kronospan OSB3 panel
Parameter Unit A1-A3 A4 A5 C1 C2 C3 C4 D
HWD kg 7.11E-03 1.19E-03 2.1E-04 3.94E-07 2.07E-04 1.27E-04 5.58E-05 -3.26E-03
NHWD kg 6.7E+01 4.6E+01 1.45E+01 1.81E-03 4.07E+00 9.05E-01 1.08E+02 -5.49E+00
RWD kg 1.45E-02 3.33E-03 1.41E-04 3.79E-06 5.36E-04 1.04E-03 1.77E-04 -1.56E-03
CRU kg 0 0 0 0 0 0 0 0
MFR kg 0 0 0 0 0 3.62E+02 0 0
MER kg 0 0 0 0 0 0 0 0
EEE MJ 0 0 0 0 0 0 0 0
EET MJ 0 0 8.44E+02 0 0 8.82E+02 1.37E+03 0
4 Environmental Product Declaration - Kronospan Luxembourg S.A. - Oriented Strand Board (OSB)
HWD = Hazardous waste disposed; NHWD = Non-hazardous waste disposed; RWD = Radioactive waste disposed; CRU = Components for re-use;
MFR = Materials for recycling; MER = Materials for energy recovery; EEE = Exported electrical energy; EET = Exported thermal energy
RESULTS OF THE LCA – additional impact categories according to EN 15804+A2-optional:
1 m3 Kronospan OSB3 panel
Parameter Unit A1-A3 A4 A5 C1 C2 C3 C4 D
Disease
PM 7.84E-05 3.71E-06 3.54E-07 3.84E-10 4.51E-07 2.91E-07 4.16E-07 -9.61E-07
incidence
IR kBq U235 eq 1.26E+01 2.13E+00 1.18E-01 4.6E-03 3.44E-01 1.26E+00 1.3E-01 -1.03E+00
ETP-fw CTUe 1.15E+04 3.84E+02 1.08E+02 3.28E-01 6.18E+01 1.02E+02 4.03E+01 -3.12E+02
HTP-c CTUh 2.88E-06 1.06E-08 2.91E-08 1.01E-11 2E-09 2.15E-08 2.97E-08 -3.93E-08
HTP-nc CTUh 3.15E-05 4.21E-07 1.25E-07 3.22E-10 6.48E-08 1.41E-07 1.07E-07 -9.94E-07
SQP SQP 3.34E+04 5.63E+02 2.4E+01 9.4E-02 5.44E+01 2.7E+01 6.52E+01 -1.79E+04
PM = Potential incidence of disease due to PM emissions; IR = Potential Human exposure efficiency relative to U235; ETP-fw = Potential comparative
Toxic Unit for ecosystems; HTP-c = Potential comparative Toxic Unit for humans (cancerogenic); HTP-nc = Potential comparative Toxic Unit for humans
(not cancerogenic); SQP = Potential soil quality index
Disclaimer 1 – for the indicator “Potential Human exposure efficiency relative to U235”. This impact category deals mainly with the
eventual impact of low-dose ionizing radiation on human health of the nuclear fuel cycle. It does not consider effects due to possible
nuclear accidents, occupational exposure or radioactive waste disposal in underground facilities. Potential ionizing radiation from the
soil, radon and from some construction materials is also not measured by this indicator.
Disclaimer 2 – for the indicators “abiotic depletion potential for non-fossil resources”, “abiotic depletion potential for fossil resources”,
“water (user) deprivation potential, deprivation-weighted water consumption”, “potential comparative toxic unit for ecosystems”,
“potential comparative toxic unit for humans – cancerogenic”, “Potential comparative toxic unit for humans - not cancerogenic”,
“potential soil quality index”. The results of this environmental impact indicator shall be used with care as the uncertainties on these
results are high as there is limited experience with the indicator.
References
Standards Rapport d'étude Volet 2 – Prise en compte de la fin de vie des
produits bois. Convention DHUP/CSTB 2009 Action 33 – Sous
EN 15804:2012+A2:2019+AC:2021 action 5. ACV & Déclarations environnementales pour des
Sustainability of construction works — Environmental Product produits et composants de la construction bois.
Declarations — Core rules for the product category of
construction products. FCBA (2019)
Fiche de déclaration environmentale et sanitaire (FDES) –
EN 13986:2004 + A1:2015 Panneaux de lamelles de bois minces orientées OSB (oriented
Wood-based panels for use in construction - Characteristics, strand board) de type 3 (panneaux travaillants utilisés en milieu
evaluation of conformity and marking humide) bruts. Epaisseur déclarée : 18 mm. FDES collective 2-
90 :2018.
EN 300
Oriented Strand Boards (OSB) - Definitions, Classification and FCBA (2022a)
Specifications. Fiche de déclaration environmentale et sanitaire (FDES) –
Panneaux de lamelles de bois minces orientées OSB (oriented
ISO 14025 strand board) de type 3 (panneaux travaillants utilisés en milieu
EN ISO 14025:2011, Environmental labels and declarations — humide) bruts. Epaisseur déclarée : 12 mm. FDES collective
Type III environmental declarations — Principles and 132289692502022.
procedures.
FCBA (2022b)
Further References Fiche de déclaration environmentale et sanitaire (FDES) –
Panneaux de fibres MDF (medium-density fibrebord) utilisés en
PCR 2021, Part A milieu humide bruts. Epaisseur déclarée : 18 mm. FDES
PCR Guidance-Texts for Building-Related Products and collective 182289782502022.
Services: Calculation Rules for the Life Cycle Assessment and
Requirements on the Project Report according to EN FCBA (2022c)
15804+A2:2019 Fiche de déclaration environmentale et sanitaire (FDES) –
Panneaux de fibres MDF (medium-density fibrebord) utilisés en
PCR 2023, Part B milieu humide bruts. Epaisseur déclarée : 19 mm. FDES
PCR-Guidances-Texts for Building-Related Products and collective 341289752502022.
Services. Part B: Requirements on the EPD for Wood based
panels SimaPro software and ecoinvent database:2021
SimaPro software ecoinvent database, version 3.8, 2021
FCBA (2012)
5 Environmental Product Declaration - Kronospan Luxembourg S.A. - Oriented Strand Board (OSB)
Publisher
Institut Bauen und Umwelt e.V. +49 (0)30 3087748- 0
Hegelplatz 1 info@ibu-epd.com
10117 Berlin www.ibu-epd.com
Germany
Programme holder
Institut Bauen und Umwelt e.V. +49 (0)30 3087748- 0
Hegelplatz 1 info@ibu-epd.com
10117 Berlin www.ibu-epd.com
Germany
Author of the Life Cycle Assessment
Luxembourg Institute of Science and Technology 00352-275888-1
(LIST) info@list.lu
Avenue des Hauts-Fourneaux 5 www.list.lu
4362 Esch/Alzette
Luxembourg
Owner of the Declaration
Kronospan Luxembourg S.A. +352590311214
Rue GadderScheier 1 j.guerlot@kronospan.lu
4984 Soleuvre www.kronospan.lu
Luxembourg
6 Environmental Product Declaration - Kronospan Luxembourg S.A. - Oriented Strand Board (OSB)
