ENVIRONMENTAL PRODUCT DECLARATION
as per ISO 14025 and EN 15804+A2
Owner of the Declaration Kvadrat Acoustics A/S
Programme holder Institut Bauen und Umwelt e.V. (IBU)
Publisher Institut Bauen und Umwelt e.V. (IBU)
Declaration number EPD-KVC-20210256-IAC1-EN
Issue date 09.12.2021
Valid to 08.12.2026
SC Broadline product
Kvadrat Acoustics A/S
www.ibu-epd.com | https://epd-online.com
Umwelt Produktdeklaration Name des Herstellers – Name des Produkts
General Information
Kvadrat Acoustics A/S SC Broadline product
Programme holder Owner of the declaration
IBU – Institut Bauen und Umwelt e.V. Kvadrat Acoustics A/S
Panoramastr. 1 Orient Plads 1, 1.
10178 Berlin DK-2150 Nordhavn
Germany
Declaration number Declared product / declared unit
EPD-KVC-20210256-IAC1-EN 1m2 configurable acoustic frame system
This declaration is based on the product Scope:
category rules: The declaration covers a model of configurable textile
Textile covered acoustic frame systems, 01.2018 covered acoustic frame systems from the company
(PCR checked and approved by the SVR) Kvadrat Soft Cells. The model is named Broadline and
the declaration includes fitting systems for installing the
frames. The product is assembled at a production site
Issue date
in Gadki, Poland, and the production data was
09.12.2021
collected for the year 2020.
Valid to
The owner of the declaration shall be liable for the
08.12.2026
underlying information and evidence; the IBU shall not
be liable with respect to manufacturer information, life
cycle assessment data and evidences.
The EPD was created according to the specifications
of EN 15804+A2. In the following, the standard will be
simplified as EN 15804.
Verification
The standard EN 15804 serves as the core PCR
Independent verification of the declaration and data
according to ISO 14025:2010
Dipl. Ing. Hans Peters internally x externally
(chairman of Institut Bauen und Umwelt e.V.)
Dr. Alexander Röder Dr.-Ing. Nikolay Minkov
(Managing Director Institut Bauen und Umwelt e.V.)) (Independent verifier)
Product
Product description/Product definition the countries and the corresponding national
specifications.
As a general rule, the configurable textile covered
acoustic frame system serves as a sound control
system, and adds to the aesthetic design of interior Application
walls and ceilings. The application is sound control and the products add
to the aesthetic design of interior walls and ceilings.
The system is based on the following principles: The products can be applied in many different markets,
The front textile membrane is attached to a specially architectural needs and acoustic environments.
designed frame profile with an integrated tensioning Examples of these are offices, auditoriums, libraries,
system, which is then positioned as a panel on the wall hotels and public spaces.
or in the ceiling using various types of fitting systems
such as for example magnets, wires (for suspended Technical Data
ceilings), while hinges can also be used if regular
subsequent access behind the panel is desired.
As part of the Broadline model of frame systems a
layer of acoustic padding in the form of mineral wool is Constructional data
used for sound absorption inside the panels. Name Value Unit
Sound absorption coefficient cf. ISO-
0.1 - 1 -
The frame systems come in customised sizes and can 354
be combined to cover a given surface area. 6000*30
Dimensions max. (l x w x h) mm
00*49
For the use and application of the product the 2000*50
Dimensions min. (l x w x h) * mm
respective national provisions at the place of use 0*49
apply, in Germany for example the Building Codes of Fire performance cf. EN-13501-1 A1 to E -
2 Environmental Product Declaration Kvadrat Soft Cells – KSC Broadline
* Smaller sizes are available from KSC, but are not accounts
covered by the EPD. Front textiles 6 wt-%
Other materials 9 wt-%
Performance data of the product with respect to its
characteristics in accordance with the relevant This product does not contain substances listed in the
technical provision (No CE-marking). candidate list (date: 25.06.2020) exceeding 0.1
percentage by mass.
Base materials/Ancillary materials
Reference service life
The content stated in the table refers to the product not The RSL is not required for the EPD because the use
counting packaging materials stage modules are not declared.
Name Value Unit
Main profile, bracing profile, binding
54 wt-%
profile of aluminium
Sound absorber made of mineral wool 31 wt-%
LCA: Calculation rules
Declared Unit Content of textile membrane
6 %
Some product components come in a number of (based on weight)
different varieties, but more than 90% of the products Deviation from frame (max. kg/m²) 46 %
use only a few of these varieties. In this case the few Panel size average 2 m2
varieties are applied to represent the full range. For
example, this applies to the front textiles, where a
polyester and a wool textile are applied in the average
frame system although some products (<10%) apply
other front textile materials. System boundary
The EPD is of the type cradle-to-gate with options,
There are five overall fitting systems, which are modules C1-C4 and D.
included in the product declaration by calculating an
arithmetic average. The same applies to the average Comparability
size of the panels. Basically, a comparison or an evaluation of EPD data
is only possible if all the data sets to be compared
Declared unit were created according to EN 15804 and the building
Name Value Unit context, respectively the product-specific
Declared unit 1 m2 characteristics of performance, are taken into account.
Conversion factor to 1 kg 6.4 kg/m2
Content of frame (based on GaBi Sphera version 2021.2 background databases
54 %
weight) were applied
LCA: Scenarios and additional technical information
Characteristic product properties
Information on biogenic Carbon Installation into the building (A5)
Module A5 is not declared. However, the packaging
In the Broadline products, the total mass of biogenic materials are disposed of in A5 and therefore a
carbon-containing materials is less than 5 % and is scenario for this is included.
therefore omitted. Name Value Unit
Plastic packaging for recycling 0.37 kg
Cardboard packaging for incineration 0.315 kg
Information on describing the biogenic Carbon
Content at factory gate
Name Value Unit Use or application of the installed product (B1) see
Biogenic Carbon Content in section 2.12 "Use"
0.25 kg C
accompanying packaging (cardboard) Name Value Unit
Maintenance (B2)
Only modules A1-A3 are declared. Name Value Unit
Information on maintenance - -
The manufacturing activities at the production site are Number/
Maintenance cycle -
assembly related and done mostly by hand. This RSL
includes cutting, assembly with the use of hand tools, Water consumption - m3
quality control and packaging. Auxiliary - kg
Other resources - kg
Electricity consumption - kWh
Transport to the building site (A4) Other energy carriers - MJ
Material loss - kg
Name Value Unit
Repair (B3)
3 Environmental Product Declaration Kvadrat Soft Cells – KSC Broadline
Name Value Unit
Information on the repair process - -
Information on the inspection process - -
Number/
Repair cycle -
RSL
Water consumption - m3
Auxiliary - kg
Other resources - kg
Electricity consumption - kWh
Other energy carriers - MJ
Material loss - kg
Replacement (B4) / Refurbishment (B5)
Name Value Unit
Number/
Replacement cycle -
RSL
Electricity consumption - kWh
Litres of fuel - l/100km
Replacement of worn parts - kg
Reference service life
Name Value Unit
Reference service life - a
Operational energy use (B6) and Operational water
use (B7)
Name Value Unit
Water consumption - m3
Electricity consumption - kWh
Other energy carriers - MJ
Equipment output - kW
End of life (C1 - C4)
Name Value Unit
Collected separately 6.38 kg
Recycling 4.03 kg
Landfilling 2.34 kg
Reuse, recovery and/or recycling potentials (D),
relevant scenario information
Name Value Unit
Replaced primary aluminium 2.29 kg
Replaced primary steel 0.09 kg
Replaced primary galvanized steel 0.24 kg
Some zinc and neodymium are also recycled at end-
of-life, but no replacement of primary metal was
included for these metals.
4 Environmental Product Declaration Kvadrat Soft Cells – KSC Broadline
LCA: Results
DESCRIPTION OF THE SYSTEM BOUNDARY (X = INCLUDED IN LCA; ND = MODULE OR INDICATOR NOT
DECLARED; MNR = MODULE NOT RELEVANT)
BENEFITS AND
CONSTRUCTI LOADS
PRODUCT STAGE ON PROCESS USE STAGE END OF LIFE STAGE BEYOND THE
STAGE SYSTEM
BOUNDARIES
5 Environmental Product Declaration Kvadrat Soft Cells – KSC Broadline
lairetam
waR
ylppus tropsnarT
gnirutcafunaM
eht
morf
tropsnarT
etis
eht
ot
etag
ylbmessA esU
ecnanetniaM
riapeR
tnemecalpeR tnemhsibrufeR
ygrene
lanoitarepO esu
retaw
lanoitarepO esu
noitcurtsnoc-eD
noitilomed tropsnarT
gnissecorp
etsaW
lasopsiD -esueR -yrevoceR -gnilcyceR laitnetop
A1 A2 A3 A4 A5 B1 B2 B3 B4 B5 B6 B7 C1 C2 C3 C4 D
X X X ND ND ND ND MNR MNR MNR ND ND X X X X X
RESULTS OF THE LCA - ENVIRONMENTAL IMPACT according to EN 15804+A2: 1 m² Kvadrat Soft Cells
SC Broadline product
Core Indicator Unit A1 A2 A3 C1 C2 C3 C4 D
GWP-total [kg CO2-Eq.] 3.13E+1 2.47E-1 3.99E+0 0.00E+0 3.79E-2 1.72E-2 6.28E-1 -2.00E+1
GWP-fossil [kg CO2-Eq.] 3.09E+1 2.46E-1 4.13E+0 0.00E+0 3.76E-2 1.71E-2 8.18E-2 -2.00E+1
GWP-biogenic [kg CO2-Eq.] 3.33E-1 2.44E-4 -1.46E-1 0.00E+0 -4.79E-5 5.58E-6 5.46E-1 2.08E-3
GWP-luluc [kg CO2-Eq.] 2.52E-2 3.33E-4 1.62E-3 0.00E+0 3.08E-4 1.18E-4 1.10E-4 -7.10E-3
ODP [kg CFC11-Eq.] 1.92E-7 2.18E-17 3.66E-12 0.00E+0 4.80E-18 4.44E-17 1.82E-16 -5.58E-14
AP [mol H+-Eq.] 1.53E-1 9.53E-4 6.54E-3 0.00E+0 1.21E-4 1.66E-4 3.53E-4 -7.51E-2
EP-freshwater [kg PO4-Eq.] 7.62E-4 1.52E-7 2.02E-5 0.00E+0 1.12E-7 4.88E-8 5.32E-6 -9.26E-6
EP-marine [kg N-Eq.] 1.01E-1 4.32E-4 2.27E-3 0.00E+0 5.58E-5 8.12E-5 3.31E-4 -1.29E-2
EP-terrestrial [mol N-Eq.] 3.28E-1 4.74E-3 2.34E-2 0.00E+0 6.23E-4 8.92E-4 1.11E-3 -1.40E-1
POCP [kg NMVOC-Eq.] 6.58E-2 1.18E-3 6.88E-3 0.00E+0 1.09E-4 2.37E-4 4.69E-4 -3.86E-2
ADPE [kg Sb-Eq.] 1.92E-4 9.86E-9 4.06E-7 0.00E+0 2.86E-9 1.88E-8 4.71E-9 -1.74E-5
ADPF [MJ] 4.25E+2 3.32E+0 8.04E+1 0.00E+0 5.00E-1 3.34E-1 7.98E-1 -2.64E+2
[m³ world-Eq
WDP 6.85E+0 6.19E-4 1.30E-1 0.00E+0 3.26E-4 3.20E-3 5.17E-3 -1.32E+0
deprived]
GWP = Global warming potential; ODP = Depletion potential of the stratospheric ozone layer; AP = Acidification potential of land and water; EP =
Caption Eutrophication potential; POCP = Formation potential of tropospheric ozone photochemical oxidants; ADPE = Abiotic depletion potential for non-
fossil resources; ADPF = Abiotic depletion potential for fossil resources; WDP = Water (user) deprivation potential
RESULTS OF THE LCA - INDICATORS TO DESCRIBE RESOURCE USE according to EN 15804+A2: 1 m²
Kvadrat Soft Cells SC Broadline product
Indicator Unit A1 A2 A3 C1 C2 C3 C4 D
PERE [MJ] 1.59E+2 3.69E-2 9.56E+0 0.00E+0 2.79E-2 2.46E-2 8.23E-2 -8.49E+1
PERM [MJ] 4.67E+0 0.00E+0 4.50E+0 0.00E+0 0.00E+0 0.00E+0 0.00E+0 0.00E+0
PERT [MJ] 1.63E+2 3.69E-2 1.41E+1 0.00E+0 2.79E-2 2.46E-2 8.23E-2 -8.49E+1
PENRE [MJ] 4.22E+2 3.33E+0 6.04E+1 0.00E+0 5.01E-1 3.35E-1 7.99E-1 -2.64E+2
PENRM [MJ] 3.54E+0 0.00E+0 2.00E+1 0.00E+0 0.00E+0 0.00E+0 0.00E+0 0.00E+0
PENRT [MJ] 4.26E+2 3.33E+0 8.04E+1 0.00E+0 5.01E-1 3.35E-1 7.99E-1 -2.64E+2
SM [kg] 1.81E+0 0.00E+0 1.22E-1 0.00E+0 1.22E-1 0.00E+0 0.00E+0 0.00E+0
RSF [MJ] 0.00E+0 0.00E+0 0.00E+0 0.00E+0 0.00E+0 0.00E+0 0.00E+0 0.00E+0
NRSF [MJ] 0.00E+0 0.00E+0 0.00E+0 0.00E+0 0.00E+0 0.00E+0 0.00E+0 0.00E+0
FW [m³] 4.24E-1 4.65E-5 8.42E-3 0.00E+0 3.19E-5 9.21E-5 1.55E-4 -1.80E-1
PERE = Use of renewable primary energy excluding renewable primary energy resources used as raw materials; PERM = Use of
renewable primary energy resources used as raw materials; PERT = Total use of renewable primary energy resources; PENRE = Use of
non-renewable primary energy excluding non-renewable primary energy resources used as raw materials; PENRM = Use of non-
Caption
renewable primary energy resources used as raw materials; PENRT = Total use of non-renewable primary energy resources; SM = Use
of secondary material; RSF = Use of renewable secondary fuels; NRSF = Use of non-renewable secondary fuels; FW = Use of net fresh
water
RESULTS OF THE LCA – WASTE CATEGORIES AND OUTPUT FLOWS according to EN 15804+A2:
1 m² Kvadrat Soft Cells SC Broadline product
Indicator Unit A1 A2 A3 C1 C2 C3 C4 D
HWD [kg] 2.79E-4 4.32E-11 9.43E-8 0.00E+0 2.52E-11 1.87E-11 1.15E-10 -4.98E-5
NHWD [kg] 5.71E+0 3.56E-4 5.36E-1 0.00E+0 7.44E-5 8.96E-5 2.24E+0 -4.25E+0
RWD [kg] 2.13E-2 2.98E-6 6.01E-4 0.00E+0 6.06E-7 4.31E-6 8.84E-6 -1.96E-2
CRU [kg] 0.00E+0 0.00E+0 0.00E+0 0.00E+0 0.00E+0 0.00E+0 0.00E+0 0.00E+0
MFR [kg] 0.00E+0 0.00E+0 0.00E+0 0.00E+0 0.00E+0 4.03E+0 0.00E+0 0.00E+0
MER [kg] 0.00E+0 0.00E+0 0.00E+0 0.00E+0 0.00E+0 0.00E+0 0.00E+0 0.00E+0
EEE [MJ] 0.00E+0 0.00E+0 0.00E+0 0.00E+0 0.00E+0 0.00E+0 0.00E+0 0.00E+0
EET [MJ] 0.00E+0 0.00E+0 0.00E+0 0.00E+0 0.00E+0 0.00E+0 0.00E+0 0.00E+0
HWD = Hazardous waste disposed; NHWD = Non-hazardous waste disposed; RWD = Radioactive waste disposed; CRU = Components
Caption for re-use; MFR = Materials for recycling; MER = Materials for energy recovery; EEE = Exported electrical energy; EET = Exported
thermal energy
RESULTS OF THE LCA – additional impact categories according to EN 15804+A2-optional:
1 m² Kvadrat Soft Cells SC Broadline product
Indicator Unit A1 A2 A3 C1 C2 C3 C4 D
[Disease
PM 1.69E-6 3.33E-9 7.03E-8 0.00E+0 6.53E-10 3.73E-9 3.99E-9 -7.76E-7
Incidence]
[kBq U235-
IRP 5.62E+0 4.08E-4 9.20E-2 0.00E+0 8.67E-5 6.83E-4 1.11E-3 -4.26E+0
Eq.]
ETP-fw [CTUe] 7.58E+2 2.41E+0 2.27E+1 0.00E+0 3.61E-1 2.31E-1 1.17E+0 -9.88E+1
HTP-c [CTUh] 1.86E-7 4.54E-11 7.87E-10 0.00E+0 7.29E-12 4.96E-12 5.18E-11 -1.42E-8
HTP-nc [CTUh] 6.80E-7 2.23E-9 4.18E-8 0.00E+0 4.29E-10 2.97E-10 5.73E-9 -2.06E-7
SQP [-] 3.44E+2 1.89E-1 7.50E+1 0.00E+0 1.72E-1 7.45E-2 1.07E-1 -1.66E+1
PM = Potential incidence of disease due to PM emissions; IR = Potential Human exposure efficiency relative to U235; ETP-fw = Potential
Caption comparative Toxic Unit for ecosystems; HTP-c = Potential comparative Toxic Unit for humans (cancerogenic); HTP-nc = Potential
comparative Toxic Unit for humans (not cancerogenic); SQP = Potential soil quality index
It is noted that the ODP, EP-freshwater and ADPE results are sensitive to the choice of a suspension system.
Particularly, these results may increase significantly if the linear magnet suspension system is used.
Use of secondary material includes aluminium, cardboard, stainless steel and zinc. Use of secondary fuels all
come from secondary datasets as no secondary fuels are used at the KSC manufacturing site.
References
ISO 354 ISO 14025
ISO 354, 2013: Acoustics - Measurement of sound DIN EN ISO 14025:2011-10, Environmental labels and
absorption in a reverberation room. declarations — Type III environmental declarations —
Principles and procedures.
IBU PCR 2018, Part B
Requirements on the EPD for Textile covered acoustic EN 15804
frame systems. Version 1.0; 01-2018. EN 15804:2019+A2 (in press), Sustainability of
construction works — Environmental Product
IBU PCR 2019, Part A Declarations — Core rules for the product category of
The Product Category Rules for Building-Related construction products.
Products and Services, Part A: Calculation Rules for
the Life Cycle Assessment and Requirements on the
Project Report according to EN 15804+A2:2019,
Version 1.0. from Institut Bauen und Umwelt e.V. ECHA Candidate List
(IBU); List of substances of very high concern considered for
approval (status 25.06.2020) according to Article 59
IBU 2021 para. 10 of the REACH Regulation. European
Institut Bauen und Umwelt e.V.: General Instructions Chemicals Agency
for the EPD programme of Institut Bauen und Umwelt
e.V. Version 2.0, Berlin: Institut Bauen und Umwelt GaBi LCA software and database
e.V., 2021. www.ibu-epd.com. The LCA modelling software is GaBi program version
10.5.1.125 with corresponding databases from Sphera
EN 13501-1 Solutions GmbH. Documentation
EN13501-1, 2018: Fire classification of construction www.gabisoftware.com/support/gabi.
products and building elements - Part 1: Classification
using data from reaction to fire tests.
6 Environmental Product Declaration Kvadrat Soft Cells – KSC Broadline
Publisher
Institut Bauen und Umwelt e.V. Tel +49 (0)30 3087748- 0
Panoramastr. 1 Fax +49 (0)30 3087748- 29
10178 Berlin Mail info@ibu-epd.com
Germany Web www.ibu-epd.com
Programme holder
Institut Bauen und Umwelt e.V. Tel +49 (0)30 - 3087748- 0
Panoramastr 1 Fax +49 (0)30 – 3087748 - 29
10178 Berlin Mail info@ibu-epd.com
Germany Web www.ibu-epd.com
Author of the Life Cycle
Assessment Tel +4543250856
FORCE Technology Fax +4543250010
Park Alle 345 Mail chme@force.dk
2605 Brøndby Web www.forcetechnology.com
Denmark
Owner of the Declaration
Kvadrat Acoustics A/S Tel +4589531866
Orient Plads 1, 1 Fax -
2150 Nordhavn Mail kvadratacoustics@kvadrat.org
Denmark Web www.kvadratacoustics.com
