ENVIRONMENTAL PRODUCT DECLARATION
as per ISO 14025 and EN 15804+A2
Owner of the Declaration HALTON FOODSERVICE
Publisher Institut Bauen und Umwelt e.V. (IBU)
Programme holder Institut Bauen und Umwelt e.V. (IBU)
Declaration number EPD-HAL-20240074-IBA1-EN
Issue date 27/08/2024
Valid to 26/08/2029
KVI/F- Capture Jet™ hood with integrated makeup air
HALTON FOOD SERVICE
www.ibu-epd.com | https://epd-online.com
1. General Information
HALTON FOOD SERVICE KVI/F- Capture Jet™ hood with integrated makeup
air
Programme holder Owner of the declaration
IBU – Institut Bauen und Umwelt e.V. HALTON FOODSERVICE
Hegelplatz 1 Zone Technoparc Futura CS 80102
10117 Berlin 62402 BETHUNE Cedex
Germany France
Declaration number Declared product / declared unit
EPD-HAL-20240074-IBA1-EN 1 linear metre of KVI/F hood, used to extract heat and cooking steam for
365 days a year, for 8 hours a day, for 15 years
This declaration is based on the product category rules: Scope:
Ventilation systems for commercial kitchens, 24/01/2024 This document refers to KVI/F hood produced by HALTON
(PCR checked and approved by the SVR) FOODSERVICE in France. This EPD represents the declaration of a
specific product KVI/F Hood, with the declared unit of 1 linear metre of
hood, used to extract heat and cooking steam for 365 days a year, for 8
Issue date hours a day, for 15 years.
The data collection for the ecological assessment occurred plant specific
27/08/2024
with current annual data. Consequently, the Life Cycle Assessment is
representative for this product.
The owner of the declaration shall be liable for the underlying information
Valid to
and evidence; the IBU shall not be liable with respect to manufacturer
26/08/2029 information, life cycle assessment data and evidences.
The EPD was created according to the specifications of EN 15804+A2. In
the following, the standard will be simplified as EN 15804.
Verification
The standard EN 15804 serves as the core PCR
Independent verification of the declaration and data according to ISO
14025:2011
internally X externally
Dipl.-Ing. Hans Peters
(Chairman of Institut Bauen und Umwelt e.V.)
Florian Pronold Dr. Matthew Fishwick,
(Managing Director Institut Bauen und Umwelt e.V.) (Independent verifier)
1 Environmental Product Declaration - HALTON FOOD SERVICE - KVI/F- Capture Jet™ hood with integrated makeup air
2. Product
assembling, configuring, and testing of the hoods from pre-
2.1 Product description/Product definition made parts. The assessment covers the electricity, LPG
The Capture Jet™ technology (KVI/F) is related to the consumption for forklifts and water use needed during the
association of two sets of nozzles supplied with an extremely production process. The electricity is modelled as site-specific
low supply air volume (a maximum of 30 m³/h/m of hood). energy mixes provided by local energy companies.The waste
These nozzles fit to the lower part of the hood front as well as streams from the manufacturing site include, wastewater, wood
the sides, encircling the perimeter of the covered cooking waste, cardboard, plastic and metal scrap (stainless steel and
areas. The horizontal nozzles increase the push/pull of the galvanised steel sheets).
thermal plume and smoke from the lower part of the hood front Any production waste generated is disposed of according by
due to the Venturi effect. It provides an assist to push vapours Halton's waste contractor.
back towards the filters.
2.7 Environment and health during manufacturing
The product is manufactured from steel, electronics, aluminium, Workplace and emission limits are regularly monitored and are
plastic. far below the prescribed limits.
2.8 Product processing/Installation
The hood is installed in about 10 hours by 2 employees. The
For the placing on the market of the product in the European hood is fixed by hand to the ceiling with the help of a lifter and
Union/European Free Trade Association (EU/EFTA) (with the some fixation devices.
exception of Switzerland) Regulation (EU) No. 305/2011 (CPR)
2.9 Packaging
applies. The product needs a declaration of performance taking
into consideration EN and the CE-marking. For product protection the hoods are individually packed in a
For the application and use the respective national provisions cardboard box. All packaged products are wrapped with (low
apply. density polyethylene) PEBD/LDPE film on a wood pallet.
2.2 Application 2.10 Condition of use
The KVI/Fhood is used for professional kitchens. They can be To ensure the longevity of the product, a weekly cleaning (using
installed above the cooking appliances and is used to remove water with 1.5% soap) and annual check-up on different hood
fumes, odors, heat, humidity, and any airborne grease from the parameters (Capture jets state, lighting state, state and number
environment. of filters, k factor, exhaust rates in intake rates) are
recommended.
2.3 Technical Data
2.11 Environment and health during use
The technical properties are project-dependent (Airflow range).
The dimensions of the reference product is specified in the The products do not emit any contaminants or substances that
table below. are harmful to the environment or health during the use phase.
2.12 Reference service life
Reference service life for the cooker hoods is assumed 15
Constructional Data years.
Name Value Unit The reference service life is based on the empirical value for
Length 1000 mm the hoods when used in accordance with the care instructions.
Reference service life for the cooker hoods is assumed 15
Width 1400 mm
years.
Height 500 mm
Weight 91.2 kg 2.13 Extraordinary effects
power consumption (operation) 60 W Fire
The products are not classified as building materials (building
Performance data of the product with respect to its
products) and are not subject to DIN 4102 and EN 13501-1.
characteristics in accordance with the relevant technical
Water
provision (no CE-marking).
No water-hazardous, toxic substances are washed-out to the
environment and water.
2.4 Delivery status
The products vary in size as they are not catalogue products.
Mechanical destruction
2.5 Base materials/Ancillary materials There are no relevant environmental impacts associated with
mechanical destruction.
This product/article/at least one partial article contains other
Carcinogenic, mutagenic, reprotoxic (CMR) substances in
2.14 Re-use phase
categories 1A or 1B which are not on the candidate list,
The KVI/F are not taken back by the manufacturer for the
exceeding 0.1 percentage by mass: no.
purpose of reuse. Users can disassemble the products
repeatedly within the reference utilization period and reuse it
Biocide products were added to this construction product or it
elsewhere.
has been treated with biocide products (this then concerns a
treated product as defined by the (EU) Ordinance on Biocide 2.15 Disposal
Products No. 528/2012): no.
Disassembly of the products consists of the same steps as
assembly, in reverse order. The product falls under the Waste
2.6 Manufacture
from Electrical and Electronic Equipment (WEEE).
Manufacturing and packaging of the KVI/F hood at the
production site. In this case, manufacturing mainly refers to the 2.16 Further information
2 Environmental Product Declaration - HALTON FOOD SERVICE - KVI/F- Capture Jet™ hood with integrated makeup air
Additional information about our products can be found on Halton-website: www.halton.com.
3. LCA: Calculation rules
(Capture jets state, lighting state, filters (state and number), k
3.1 Declared Unit factor, exhaust rates in intake rates) modelled with
The declared unit is: 'The declared unit is: '1 linear metre of transportation of one technician in light commercial vehicle (100
hood, used to extract heat and cooking steam for 365 days a km). The number of check-ups depends on the hood model.
year, for 8 hours a day, for 15 years'. - 2 UV light replacements during the reference life service.
Declared unit - End-of-life treatment of 2 UV light tubes during SLR with
transportation included
Name Value Unit
Declared unit 1 rm
Module B6 et B7
Mass per Unit 91.2 kg The hood is designed for heavy duty industrial usage. To reflect
linear density 91.2 kg/rm the most average scenario the hood will be functioning 8 hours
a days 7 days a week. Electricity (B6) is required to use the
Other declared units are allowed if the conversion is shown
products.
transparently.
Modules C1-C4
3.2 System boundary The module includes the environmental impacts for dismantling
of the products and the treatment of the KVI/F hood waste until
This representative EPD follows the EPD type "cradle to grave".
the end-of-waste status (EoW) is reached, including the
The following life cycle modules are declared:
associated transports at the end of the product life cycle.
Modules A1-A3
The product is assumed to be removed manually at the same
The product stage begins with considering the production of the
time as the building is demolished. No scenario has been
necessary raw materials (metals, electronics, packaging
developed for stage C1.
materials), including all corresponding upstream chains and the
actual procurement transports.
The hood and the ceiling beam are removed separately.
Furthermore, the entire manufacturing phase was mapped,
Dismantling of product components at recycling facility. Based
including the treatment of production waste until the end-of
on the material, components are either recycled, incinerated, or
waste status (EoW) was reached.
landfilled depending on the material.
Module A4
Stage C3 represents the impact of a conventional scrap
The transport model considers a construction site in Europe.
processing site, with sorting, shearing, shredding, separation.
The scenario for the distribution stage considers a average
distance to serve the entire European area from the Halton's
Module D
plant. The quantity transported corresponds to the transport of
Identification of the benefits and costs of the product outside
products and their packaging to the construction site.
the system boundary.
Recycling of metal scrap results in credits of the respective raw
Module A5
materials for the primary material portion of the input. The loads
The hood is delivered at the right size on the installation site. It
of the waste incineration and recycling processes are assigned
is installed in about 10 hours by 2 employees. The hood is fixed
to the respective modules (A3, A5 and C3) and not to module
to the ceiling with the help of a lifter and some fixation devices.
D.
Complementary products for installation include a ceiling beam
3.3 Estimates and assumptions
in galvanised steel. This additional product is supplied by
Energy and water consumption during production could only be
Halton. Their production and packaging are considered in A1,
determined on existing products and not on the average
their transport in A3 and A4 and the end-of-life of their
product.
packaging in A5.
Others complementary products are used to fix the MUPRO 3.4 Cut-off criteria
Ceiling beam (clip, pin, screw). They must be purchased by the
Cut-off criteria follow EN15804 and PCR Part A. No flows have
installer because they depend on ceiling type (metallic,
been deliberately omitted from the system boundaries.
concrete or wood). They are not considered in this study.
3.5 Background data
The application phase considers: All background data was considered using data from the
- Transportation of material lifter to installation site Ecoinvent 3.7.1 database or literary sources.
- Waste treatment (product packaging)
3.6 Data quality
Site-specific production data has been collected for 2021 from
Modules B1 & B3-B5 & B7 the production site. The upstream and downstream processes
These modules were considered but evaluated as not relevant have been modelled based on environmental data from generic
for the products and considered as zero. Products do not databases ecoinvent. The collected data was reviewed in terms
require repair (B3)/replacement (B4)/rehabilitation (B5). of consistency, and it is estimated as good quality.
The hoods haven't significant impact for emission in indoor air 3.7 Period under review
or in water during use. The data is therefore based on 2021. All information is based
on averaged data for 12 consecutive months.
Module B2
3.8 Geographic Representativeness
- a weekly cleaning with 5L of water containing 1,5% soap.
- annual check-up by a technician on different hood parameters
3 Environmental Product Declaration - HALTON FOOD SERVICE - KVI/F- Capture Jet™ hood with integrated makeup air
Land or region, in which the declared product system is
manufactured, used or handled at the end of the product´s 3.10 Comparability
lifespan: Europe Basically, a comparison or an evaluation of EPD data is only
possible if all the data sets to be compared were created
according to EN 15804 and the building context, respectively
3.9 Allocation the product-specific characteristics of performance, are taken
Allocation has been avoided whenever possible by collecting into account. According to the EN 15804 standard,
product specific environmental data. In case of manufacturing environmental declarations for construction products may not
energy use, where allocation could not be avoided, the be comparable if they have not been prepared in accordance
consumption of electricity and water in Halton's plant were with that standard or if a different notified unit has been
allocated per working hours for assembly of each product. No used.The LCA was conducted using SimaPro 9.2.0.2. software.
other allocations were made in this assessment. The cut-off All background data was considered using data from the
end-of-life allocation approach was used throughout. ecoinvent 3.7.1 (cut-off) database or literary sources.
4. LCA: Scenarios and additional technical information
Service Life
Characteristic product properties of biogenic carbon HALTON declares a Service Life of 15 years as an empirical
The biogenic carbon content quantifies the amount of biogenic value for the hoods when used in accordance with the care
carbon in a construction product leaving the factory gate, and it instructions.
shall be separately declared for the product and for any
Maintenance (B2)
accompanying packaging.
Name Value Unit
The mass of packaging containing biogenic carbon is declared. Total number of check-up
60
during SRL
Note: 1 kg of biogenic carbon is equivalent to 44/12 kg of CO 2. Estimated distance for round
100 km
Name Value Unit trip
Biogenic carbon content of the product 0 kg.C Estimated weight of
technician doing the check 80 kg
Biogenic carbon content of associated packaging 15.2 kg.C
up.
2 replacements of UV light 5.40E-
The scenarios and assumptions applied in this study for all the kg
during SLR 01
life cycle stages included are based on data provided by Halton
3.09E m3 of water containing
and correspond to the most likely scenario. The following Weekly cleaning
+03 1,5% soap /DVR
scenarios and general assumptions were made in the studied
lifecycle stages:
Operational energy and water use (B6-B7)
Based on a 56h/week usage of the hood.
Transport to the building site (A4)
Name Value Unit
Name Value Unit
Water consumption 0 m3
Transport of distance 1631.4 km
Energy demand 175.2 kWh/year
Capacity utilization (including empty runs) ~19 %
End of life (C1-C4)
Installation into the building (A5)
Name Value Unit
Name Value Unit
Transport to treatment site 50 km
Material loss 0 %
The following end of life scenarios are considered for the
The following end of life scenarios are considered for product:
packaging:
NHW Plastic : 1.27E+00 kg → 41% recycling, 37% incineration
NHW Plastic : 1.43E+00 kg → 41% recycling, 37% incineration without energy recovery, 22% landfill
without energy recovery, 22% landfill. NHW Steel : 8.93E+01 kg → 90% recycling, 10% landfill
NHW Glass : 6.97E-01 kg → 100% landfill
NHW Cardboard : 4.33E+00 kg → 82% recycling, 9% NHW WEE : 2.59E+00 kg → 74.7% recycling, 1.8% reuse,
incineration without energy recovery, 9% landfill. 9.7% incineration without energy recovery, 13.8% landfill
NHW Wood : 3.00E+01 kg → 31% recycling, 31% incineration
without energy recovery, 38% landfill.
4 Environmental Product Declaration - HALTON FOOD SERVICE - KVI/F- Capture Jet™ hood with integrated makeup air
5. LCA: Results
The following table shows the result of the LCA for 1 m of a KVI/F hood.
DESCRIPTION OF THE SYSTEM BOUNDARY (X = INCLUDED IN LCA; MND = MODULE OR INDICATOR NOT DECLARED; MNR
= MODULE NOT RELEVANT)
Benefits and
Construction loads beyond
Product stage Use stage End of life stage
process stage the system
boundaries
la ire ta m w a Ry lp p u s tro p s n a rT g n iru tc a fu n a M e h t m o rf tro p s n a rTe tis e h t o t e ta g y lb m e s s A e s U e c n a n e tn ia M ria p e R tn e m e c a lp e R tn e m h s ib ru fe R y g re n e la n o ita re p Oe s u re ta w la n o ita re p Oe s u n o itc u rts n o c -e Dn o itilo m e d tro p s n a rT g n is s e c o rp e ts a W la s o p s iD -e s u e R-y re v o c e R-g n ilc y c e Rla itn e to p
A1 A2 A3 A4 A5 B1 B2 B3 B4 B5 B6 B7 C1 C2 C3 C4 D
X X X X X MND X MNR MNR MNR X MND X X X X X
RESULTS OF THE LCA - ENVIRONMENTAL IMPACT according to EN 15804+A2: 1 m KVI/F Hood
Parameter Unit A1-A3 A4 A5 B2 B6 C1 C2 C3 C4 D
GWP-total kg CO 2 eq 1.08E+03 2.49E+01 1.14E+02 1.44E+03 1.08E+03 0 7.59E-01 3.25E+00 2.06E+00 -1.34E+02
GWP-fossil kg CO 2 eq 1.13E+03 2.49E+01 4.6E+01 1.27E+03 1.07E+03 0 7.58E-01 1.7E+00 1.9E+00 -1.33E+02
GWP-
biogenic kg CO 2 eq -4.61E+01 9.59E-03 6.8E+01 2.1E+01 6.2E+00 0 2.92E-04 1.55E+00 1.62E-01 -3.21E-01
GWP-luluc kg CO 2 eq 1.39E+00 8.53E-03 2.17E-02 1.45E+02 2.23E+00 0 2.6E-04 1.13E-03 3.61E-05 -6.45E-02
ODP kg CFC11 eq 6E-05 5.66E-06 8.64E-06 2.09E-04 5.45E-05 0 1.72E-07 1.9E-07 2.96E-08 -5.3E-06
AP mol H+ eq 6.6E+00 6.92E-02 1.55E-01 7.41E+00 5.86E+00 0 2.11E-03 8.92E-03 1.01E-03 -4.87E-01
EP-
kg P eq 7.76E-02 1.87E-04 4.88E-04 7.82E-01 1.14E-01 0 5.68E-06 6.8E-05 3.24E-06 -6.71E-03
freshwater
EP-marine kg N eq 1.25E+00 1.41E-02 5.78E-02 3.03E+00 7.82E-01 0 4.29E-04 4.14E-03 5.87E-04 -1.15E-01
EP-terrestrial mol N eq 1.35E+01 1.57E-01 4.75E-01 2.4E+01 8.99E+00 0 4.78E-03 3.15E-02 4.26E-03 -1.23E+00
kg NMVOC
POCP 3.88E+00 6E-02 1.51E-01 6.91E+00 2.45E+00 0 1.83E-03 8.43E-03 1.2E-03 -6.05E-01
eq
ADPE kg Sb eq 4.97E-02 9.15E-05 2.61E-04 2.5E-02 9.76E-03 0 2.79E-06 5.88E-05 2.84E-07 -1.93E-04
ADPF MJ 1.48E+04 3.78E+02 6.03E+02 1.79E+04 2.27E+04 0 1.15E+01 1.66E+01 1.93E+00 -1.34E+03
m3 world eq
WDP 3.69E+02 1.09E+00 2.29E+00 7.67E+02 2.33E+02 0 3.32E-02 1.31E-01 1.47E-01 2.65E-01
deprived
GWP = Global warming potential; ODP = Depletion potential of the stratospheric ozone layer; AP = Acidification potential of land and water; EP =
Eutrophication potential; POCP = Formation potential of tropospheric ozone photochemical oxidants; ADPE = Abiotic depletion potential for non-fossil
resources; ADPF = Abiotic depletion potential for fossil resources; WDP = Water (user) deprivation potential)
RESULTS OF THE LCA - INDICATORS TO DESCRIBE RESOURCE USE according to EN 15804+A2: 1 m KVI/F Hood
Parameter Unit A1-A3 A4 A5 B2 B6 C1 C2 C3 C4 D
PERE MJ 2.6E+03 5.16E+00 1.26E+01 2.13E+03 4.09E+03 0 1.57E-01 2.01E+00 3.75E-02 -2.29E+02
PERM MJ 5.67E+02 0 -2.15E+02 0 0 0 0 0 0 0
PERT MJ 3.16E+03 5.16E+00 -2.03E+02 2.13E+03 4.09E+03 0 1.57E-01 2.01E+00 3.75E-02 -2.29E+02
PENRE MJ 1.47E+04 3.78E+02 6.28E+02 1.81E+04 2.23E+04 0 1.15E+01 1.64E+01 1.93E+00 -1.34E+03
PENRM MJ 1.09E+02 0 -2.52E+01 0 0 0 0 0 -4.79E+00 0
PENRT MJ 1.48E+04 3.77E+02 6.02E+02 1.8E+04 2.23E+04 0 1.15E+01 1.64E+01 -2.85E+00 -1.33E+03
SM kg 0 0 0 0 0 0 0 0 0 0
RSF MJ 0 0 0 0 0 0 0 0 0 0
NRSF MJ 0 0 0 0 0 0 0 0 0 0
FW m3 1.34E+01 5.16E-02 1.19E-01 2.64E+01 1.88E+01 0 1.57E-03 8.99E-03 3.78E-03 -1.32E-01
PERE = Use of renewable primary energy excluding renewable primary energy resources used as raw materials; PERM = Use of renewable primary
energy resources used as raw materials; PERT = Total use of renewable primary energy resources; PENRE = Use of non-renewable primary energy
excluding non-renewable primary energy resources used as raw materials; PENRM = Use of non-renewable primary energy resources used as raw
materials; PENRT = Total use of non-renewable primary energy resources; SM = Use of secondary material; RSF = Use of renewable secondary fuels;
NRSF = Use of non-renewable secondary fuels; FW = Use of net fresh water
RESULTS OF THE LCA – WASTE CATEGORIES AND OUTPUT FLOWS according to EN 15804+A2:
1 m KVI/F Hood
Parameter Unit A1-A3 A4 A5 B2 B6 C1 C2 C3 C4 D
HWD kg 5.1E+02 2.6E-01 3.31E+00 7.39E+01 2.51E+01 0 7.91E-03 4.86E-01 8.43E-02 -1.32E+01
NHWD kg 1.4E+03 2.15E+01 3.8E+01 9.98E+02 4.1E+02 0 6.55E-01 2.61E+00 9.14E+00 -3.1E+02
RWD kg 5.36E-02 2.58E-03 4.02E-03 1.03E-01 1.6E-01 0 7.87E-05 1.25E-04 1.1E-05 -2.45E-03
CRU kg 0 0 0 7.39E+01 2.51E+01 0 0 4.86E-01 0 -1.32E+01
MFR kg 3.32E+01 0 1.34E+01 9.98E+02 4.1E+02 0 0 2.61E+00 0 -3.1E+02
MER kg 0 0 0 1.03E-01 1.6E-01 0 0 1.25E-04 0 -2.45E-03
EEE MJ 0 0 0 0 0 0 0 4.67E-02 0 0
5 Environmental Product Declaration - HALTON FOOD SERVICE - KVI/F- Capture Jet™ hood with integrated makeup air
EET MJ 0 0 0 0 0 0 0 0 0 0
HWD = Hazardous waste disposed; NHWD = Non-hazardous waste disposed; RWD = Radioactive waste disposed; CRU = Components for re-use;
MFR = Materials for recycling; MER = Materials for energy recovery; EEE = Exported electrical energy; EET = Exported thermal energy
RESULTS OF THE LCA – additional impact categories according to EN 15804+A2-optional:
1 m KVI/F Hood
Parameter Unit A1-A3 A4 A5 B2 B6 C1 C2 C3 C4 D
Disease
PM 7.16E-05 1.57E-06 2.11E-06 1.19E-04 1.55E-05 0 4.78E-08 1.46E-07 1.69E-08 -8.32E-06
incidence
IR kBq U235 eq 5.94E+01 1.66E+00 2.66E+00 7.82E+01 1.96E+02 0 5.06E-02 1.09E-01 7.23E-03 -2.27E+00
ETP-fw CTUe 3.84E+04 2.9E+02 5.97E+02 3.55E+04 1.42E+04 0 8.84E+00 2.33E+02 2.61E+01 -3.15E+03
HTP-c CTUh 1.04E-05 1.03E-08 2.54E-08 1.97E-06 4.23E-07 0 3.13E-10 3.25E-09 4.69E-10 -7.97E-07
HTP-nc CTUh 2.56E-05 2.83E-07 5.5E-07 2.23E-05 1.11E-05 0 8.63E-09 4.53E-08 7.61E-09 -2.76E-06
SQP SQP 1.97E+04 3.86E+02 4.24E+02 3.12E+04 7.3E+03 0 1.18E+01 9.97E+01 3.31E+00 -2.12E+03
PM = Potential incidence of disease due to PM emissions; IR = Potential Human exposure efficiency relative to U235; ETP-fw = Potential comparative
Toxic Unit for ecosystems; HTP-c = Potential comparative Toxic Unit for humans (cancerogenic); HTP-nc = Potential comparative Toxic Unit for humans
(not cancerogenic); SQP = Potential soil quality index
Disclaimer 1 – for the indicator “Potential Human exposure efficiency relative to U235”. This impact category deals mainly with the
eventual impact of low-dose ionizing radiation on human health of the nuclear fuel cycle. It does not consider effects due to possible
nuclear accidents, occupational exposure or radioactive waste disposal in underground facilities. Potential ionizing radiation from the
soil, radon and from some construction materials is also not measured by this indicator.
Disclaimer 2 – for the indicators “abiotic depletion potential for non-fossil resources”, “abiotic depletion potential for fossil resources”,
“water (user) deprivation potential, deprivation-weighted water consumption”, “potential comparative toxic unit for ecosystems”,
“potential comparative toxic unit for humans – cancerogenic”, “Potential comparative toxic unit for humans - not cancerogenic”,
“potential soil quality index”. The results of this environmental impact indicator shall be used with care as the uncertainties on these
results are high as there is limited experience with the indicator.
6. LCA: Interpretation
The dominance analysis shows that modules B2 and B6 are
the dominant life cycle stages in most of the categories. The
contribution of B2 is due to the transportation of a technician for
an annual check-up. Module B6 dominates most indicators due
to the energy demand for use. The modules A1-A3 have low
contributions to all categories except for the Depletion of abiotic
resources - minerals and metals. In this indicator the provision
of chromium steel has the largest contribution. The end-of-life
stage has no significant influence on the environmental
indicators. The environmental burdens from the transports
(modules A4 and C2) account for 1% of the total burdens from
the transports in all cases.
7. Requisite evidence
8. References
PCR 2020, Part A EN 15804:2012+A2:2019+AC:2021, Sustainability of
Institut Bauen und Umwelt e.V., Berlin (pub.): Product construction works — Environmental Product Declarations —
Category Rule for Construction Products from the Core rules for the product category of construction products.
range of Environmental Product Declarations of
Institute Bauen und Umwelt (IBU), Part A: Calculation ISO 14025
rules for the Life Cycle Assessment and requirements EN ISO 14025:2011, Environmental labels and declarations —
on the project report according to EN 15804+A2. Type III environmental declarations — Principles and
Version 2020-07. procedures.
www.ibu-epd.com
DIN 4102-1
PCR 2024, Part B DIN 4102-1: Fire behaviour of building materials and building
Product Category Rules for Construction Products, components - Part 1: Building materials; concepts,
Part B: Ventilations systems for commercial kitchens, requirements and tests. 1998-05
24/01/2024
DIN EN 13501-1
EN 15804 DIN EN 13501-1:2019-05: Fire classification of construction
6 Environmental Product Declaration - HALTON FOOD SERVICE - KVI/F- Capture Jet™ hood with integrated makeup air
products and building elements - Part 1: Classification using Directives 91/155/EEC, 93/67/EEC,
data from reaction to fire tests; German version EN 13501- 93/105/EC and 2000/21/EC, 2006-12.
1:2018
Biocide Guideline
/Further References Regulation (EU) No. 528/2012 of the European
Parliament and of the Council of 22 May 2012
SimaPro 9.2.0.2 concerning the making available on the market and
use of biocidal products
CPR
Directive (EU) No. 305/2011 of the European
Waste Electrical and Electronic Equipment Directive : Act Parliament and Council dated 9 March 2011
governing the requirements on utilisation and disposal of establishing harmonised conditions for marketing
WEEE. construction products and replacing Council Guideline
89/106/EEC
REACH Regulation Ecoinvent
Regulation (EC) No. 1907/2006 of the European Parliament Ecoinvent database version 3.7.1
and of the Council of 18 December 2006 concerning the
Registration, Evaluation, Authorisation and Restriction of
Chemicals (REACH), establishing a European Chemicals IBU 2021
Agency, amending Directive 1999/45/EC and repealing Council Institut Bauen und Umwelt e.V.: General Instructions for the
Regulation (EEC) No. 793/93, Commission Regulation (EC) No. EPD programme of Institut Bauen und Umwelt e.V., Version
1488/94 2.0, Berlin: Institut Bauen und Umwelt e.V., 2021
as well as Council Directive 76/769/EEC and Commission www.ibu-epd.com
7 Environmental Product Declaration - HALTON FOOD SERVICE - KVI/F- Capture Jet™ hood with integrated makeup air
Publisher
Institut Bauen und Umwelt e.V. +49 (0)30 3087748- 0
Hegelplatz 1 info@ibu-epd.com
10117 Berlin www.ibu-epd.com
Germany
Programme holder
Institut Bauen und Umwelt e.V. +49 (0)30 3087748- 0
Hegelplatz 1 info@ibu-epd.com
10117 Berlin www.ibu-epd.com
Germany
Author of the Life Cycle Assessment
CSTB 04 56 14 72 62
rue Joseph Fourier 24 cecile.magnin-feysot@cstb.fr
38400 Saint-Martin-d'Hères https://www.cstb.fr/fr/
France
Owner of the Declaration
HALTON FOODSERVICE 06.14.71.06.55
Zone Technoparc Futura CS 80102 arnaud.kazmierczak@halton.com
62402 BETHUNE Cedex https://www.halton.com/fr/
France
8 Environmental Product Declaration - HALTON FOOD SERVICE - KVI/F- Capture Jet™ hood with integrated makeup air
