ENVIRONMENTAL PRODUCT DECLARATION
as per ISO 14025 and EN 15804+A2
Owner of the Declaration dormakaba International Holding GmbH
Publisher Institut Bauen und Umwelt e.V. (IBU)
Programme holder Institut Bauen und Umwelt e.V. (IBU)
Declaration number EPD-DOR-20210247-CBA3-EN
Issue date 15.02.2022
Valid to 14.02.2027
LA GARD 700
dormakaba
www.ibu-epd.com | https://epd-online.com
General Information
dormakaba LA GARD 700
Programme holder Owner of the declaration
IBU – Institut Bauen und Umwelt e.V. dormakaba International Holding GmbH
Hegelplatz 1 DORMA Platz 1
10117 Berlin 58256 Ennepetal
Germany Germany
Declaration number Declared product / declared unit
EPD-DOR-20210247-CBA3-EN 1 LA GARD 700 Series electronic safe lock (1piece), consisting of the
following items:
- swing bolt, dual handed
- keypad with OLED display (excluding batteries and any energy supply
modules)
This declaration is based on the product category rules: Scope:
Electronic and physical Access Control Systems, 01.08.2021 This declaration is a specific product declaration for the LA GARD 700
(PCR checked and approved by the SVR) series electronic safe lock.
The underlying life cycle assessment is based on the entire life cycle of
this specific LA GARD 700 Series electronic safe lock manufactured by
Issue date dormakaba. The various technical features are outlined in chapter 2. The
products are manufactured at the dormakaba production facility in Nogales
15.02.2022
(Mexico). The year of data collection is 2021. The declared product is not
including the batteries and energy supply modules
The owner of the declaration shall be liable for the underlying information
Valid to
and evidence; the IBU shall not be liable with respect to manufacturer
14.02.2027 information, life cycle assessment data and evidences.
The EPD was created according to the specifications of EN 15804+A2. In
the following, the standard will be simplified as EN 15804.
Verification
The standard EN 15804 serves as the core PCR
Independent verification of the declaration and data according to ISO
14025:2011
internally X externally
Dipl.-Ing. Hans Peters
(Chairman of Institut Bauen und Umwelt e.V.)
Florian Pronold Dr.-Ing. Wolfram Trinius,
(Managing Director Institut Bauen und Umwelt e.V.) (Independent verifier)
1 Environmental Product Declaration - dormakaba - LA GARD 700
Product
Product description/Product definition Technical Data
LA GARD has been an industry leader in the safe lock sector Following technical specification applies for LA GARD 700
for nearly half of a century. Series:
Name Value Unit
The LA GARD 700 Series embodies the original tried-and-true
11 (2id +
features Combination length -
6-9)
and long legacy of LA GARD high-security function along with
Battery power 2x9 V
advanced
1.28” Monochrome OLED Display 128 x 64 -
technological features.
The series offers a range of features and options to fit almost Low-energy Bluetooth key fob for credential
x -
any and Time Delay Override
safe lock need. Single unified software platform for increased
x -
• Security – the electronic safe locks are designed to usability and updatable firmware
support the ever-changing needs of today's world Power supply
• Efficiency – lower total cost of ownership, fewer battery
changes, ease of use, simplified inventory management - 2 batteries 1.5 V AA L91, FR6 or via the S module (not
included in this EPD)
• Confidence – from a name you know and trust
- via the S-module: 12–24 V AC or 12–24 V DC, ≥ 0.4 A (not
• User Experience – unified software platform, feature- included in this EPD)
rich OLED display, simplified user-prompts
• Excellence – quality commitment backed by 2 year The products are not harmonised in accordance with the
warranty; extended warranty Construction Product Regulations (CPR) but in accordance with
available, world-class support, modern dormakaba other provisions for harmonisation of the EU. Compliance with
design aesthetic the European Union Directive and technical specifications:
• Display – OLED keypad featuring on-screen prompts • DIN EN 1300: 2019-05, Secure storage units -
For placing the LA GARD 700 Series electronic safe lock on the Classification for high security locks according to their
market in the European Union/European Free Trade resistance to unauthorized opening.
Association (EU/EFTA) (with the exception of Switzerland) the The products are subject to CE marking according to the
following legal provisions apply: relevant harmonization legislation.
• VdS 2344:2014-07 Base materials/Ancillary materials
• VdS 2396:2014-07 For the main product components: Lock, keypad model 703
• UL 2058:2005-06 and standard profile, the product composition of the LA GARD
• DIN EN1300:2019-05 700 Series is the following:
• Restriction of Hazardous Substances (RoHS)
Application
The LA GARD 700 Series is the ideal for commercial industries,
vault storage, government and residential/personal applications
like:
• Residential
• Commerial retail
• Quick serve restaurants
• ATM and currency exchange
• Pharmacies
• Law enforcement facilities
• Valut storage
The product includes partial articles which contain substances
• Cash recyclers
listed in the Candidate List of REACH Regulation
• Military institutions
1907/2006/EC (date: 14.06.2023) exceeding 0.1 percentage by
With five models (Models 701-705) to choose from, the series
mass: no
offers a range of features and options to fit almost any safe lock
The Candidate List can be found on the ECHA website
need. Following models are available:
address: https: echa.europa.eu/de/home.
• Model 701 – basic offering
• Model 702 – multi-user lock standard keypad Reference service life
• Model 703 – multi-user, 2-lock system, display The product is certified according to UL 2058 with testing up to
• Model 704 – multi-user, 5-lock system, display 25.000 cycles. Under normal conditions and depending on
• Model 705 – multi-user, 5-lock system, displa cycle frequency, it means an approximate duration of 7 years.
LCA: Calculation rules
Declared Unit
The declared unit is 1 piece of the product: 0.606 kg
2 Environmental Product Declaration - dormakaba - LA GARD 700
Name Value Unit
Use stage - Module B6
Declared unit 1 pce.
The use stage related to the operation of the building includes:
Mass (total system) 0.606 kg
— B6, operational energy use
Conversion factor to 1 kg 0.606 -
The potential use of electricity from the grid is declared in
module B6.
System boundary
The type of EPD is: cradle to gate with options, modules C1– End-of-life stage– Modules C1-C4 and D
C4, and module D (A1–A3 + C + D and additional modules: A4 The end-of-life stage includes:
+ A5 + B6) — C1, de-construction, demolition:
— C2, transport to waste processing;
Production - Module A1-A3 — C3, waste processing for reuse, recovery and/or recycling;
The product stage includes: — C4, disposal; including provision and all transport, provision
— A1, raw material extraction, processing and mechanical of all materials, products and related energy and water use.
treatments, processing of secondary material input (e.g.
recycling processes), Module D (Benefits and loads beyond the system boundary)
— A2, transport to the manufacturer, includes:
— A3, manufacturing and assembly including provision of all — D, recycling potentials, expressed as net impacts and
materials, products and energy, as well as waste processing up benefits.
to the end-of waste state.
Geographic Representativeness
Construction stage - Modules A4-A5 Land or region, in which the declared product system is
The construction process stage includes: manufactured, used or handled at the end of the product´s
— A4, transport to the building site; lifespan: Mexico
— A5, installation into the building; including provision of all
materials, products and energy, as well as waste processing up
Comparability
to the end-of-waste state or disposal of final residues during the
Basically, a comparison or an evaluation of EPD data is only
construction process stage.
possible if all the data sets to be compared were created
according to EN 15804 and the building context, respectively
Maintenance – Module B2
the product-specific characteristics of performance, are taken
This module includes the production and the end of life of the
into account.
batteries. The potential use of batteries is declared in module
B2.
LCA: Scenarios and additional technical information
Name Value Unit
Characteristic product properties of biogenic carbon
Use of batteries (9V batteries) 4 pieces
Information on describing the biogenic Carbon Content at
factory gate Reference service life
Name ValueUnit Name Value Unit
kg Life Span according to the manufacturer 7 a
Biogenic carbon content in product -
C
Biogenic carbon content in accompanying kg
<0.01
packaging C
Operational energy use (B6)
The use stage is declared for 7 years.
The following technical scenario information is required for the
Name Value Unit
declared modules
Electricity consumption for 1 year 0.0054 kW
Transport to the building site (A4)
Days per year in use 365 days
Name Value Unit
Stand by mode per day 23,97 h
Litres of fuel 0.00276l/100km
On mode per day 0,03 h
Capacity utilisation (including empty runs) via
55 % Stand by power 0,00015 W
medium truck
On mode power 0,375 W
Transport distance via medium truck 100 km
Two scenarios are declared:
Transport distance via plane 2800 km
- B6/1 is calculated with EU-28 electricity grid mix
The product is transported via truck and plane. The main - B6/2 is calculated with mainly US electricity grid mix (76 %)
distribution regions are Mexico and US with the calculated according to dormakaba's market
average transport distances. - Attention:
Scenarios B6/1 and B6/2 require the power supply module,
Installation into the building (A5) which is not included
in this EPD.
Name Value Unit
Waste packaging 0.0126 kg
End of life (C1-C4)
Maintenance (B2) C1: The product dismantling from the building is done manually
without environmental burden.
3 Environmental Product Declaration - dormakaba - LA GARD 700
Name Value Unit components are assumed to be incinerated with
energy recovery. Minor proportions of residues arising
Recycling 0.5016 kg
from the recycling process are landfilled (1 %).
Energy recovery 0.0971 kg
Region for the End of Life is: Global.
Landfilling 0.007671 kg
Transport to waste management 50 km Reuse, recovery and/or recycling potentials (D), relevant
scenario information
The product is disassembled in a recycling process.
Collection rate is 100 %.
Material recycling is then assumed for the metals,
electronic and electromechanics. The plastic
4 Environmental Product Declaration - dormakaba - LA GARD 700
LCA: Results
B2 declares the environmental impact for the use stage under the assumption that batteries are used.
B6 declares the environmental impact for the use stage under the assumption that electricity
from the grid (B6/1: region EU, B6/2: region mainly US) is used.
DESCRIPTION OF THE SYSTEM BOUNDARY (X = INCLUDED IN LCA; MND = MODULE OR INDICATOR NOT DECLARED; MNR
= MODULE NOT RELEVANT)
Benefits and
Construction loads beyond
Product stage Use stage End of life stage
process stage the system
boundaries
la ire ta m w a Ry lp p u s tro p s n a rT g n iru tc a fu n a M e h t m o rf tro p s n a rTe tis e h t o t e ta g y lb m e s s A e s U e c n a n e tn ia M ria p e R tn e m e c a lp e R tn e m h s ib ru fe R y g re n e la n o ita re p Oe s u re ta w la n o ita re p Oe s u n o itc u rts n o c -e Dn o itilo m e d tro p s n a rT g n is s e c o rp e ts a W la s o p s iD -e s u e R-y re v o c e R-g n ilc y c e Rla itn e to p
A1 A2 A3 A4 A5 B1 B2 B3 B4 B5 B6 B7 C1 C2 C3 C4 D
X X X X X MND X MNR MNR MNR X MND X X X X X
RESULTS OF THE LCA - ENVIRONMENTAL IMPACT according to EN 15804+A2: 1 piece LA GARD 700
Parameter Unit A1-A3 A4 A5 B2 B6/1 B6/2 C1 C2 C3 C4 D
GWP-total kg CO 2 eq 1.51E+01 1.06E+00 1.79E-02 3E-01 1.53E-02 2.26E-02 0 2.65E-03 2.51E-01 3E-04 -3.61E+00
GWP-fossil kg CO 2 eq 1.51E+01 1.06E+00 4.47E-04 3E-01 1.52E-02 2.26E-02 0 2.53E-03 2.47E-01 2.98E-04 -3.6E+00
GWP-
biogenic kg CO 2 eq 1.72E-02 1.78E-03 1.74E-02 5.26E-04 5.07E-05 9.48E-06 0 1.17E-04 3.95E-03 1.02E-06 -7.66E-03
GWP-luluc kg CO 2 eq 8.64E-03 2.22E-05 2.94E-07 2.88E-04 2.21E-05 1.13E-05 0 6.03E-08 1.4E-05 8.59E-07 -1.5E-03
kg CFC11
ODP 2.4E-10 7.72E-17 3.22E-18 5.65E-12 3.35E-16 1.09E-16 0 2.68E-19 1.25E-16 1.11E-18 -1.18E-14
eq
AP mol H+ eq 1.09E-01 4.32E-03 5E-06 9.36E-04 3.36E-05 6.32E-05 0 2.54E-06 4.45E-05 2.14E-06 -4.1E-02
EP-
kg P eq 3.26E-05 1.74E-07 6.3E-10 4.81E-07 4.06E-08 1.55E-08 0 5.42E-10 1.99E-08 5.12E-10 -4.25E-06
freshwater
EP-marine kg N eq 1.58E-02 1.92E-03 1.81E-06 2.05E-04 7.46E-06 1.17E-05 0 8.07E-07 1.01E-05 5.51E-07 -5.08E-03
EP-terrestrial mol N eq 1.71E-01 2.11E-02 2.25E-05 2.59E-03 7.84E-05 1.27E-04 0 8.97E-06 2.03E-04 6.05E-06 -5.53E-02
kg NMVOC
POCP 4.73E-02 5.48E-03 4.79E-06 5.63E-04 2.04E-05 3.37E-05 0 2.28E-06 2.79E-05 1.67E-06 -1.6E-02
eq
ADPE kg Sb eq 4.08E-03 3.01E-08 5.09E-11 1.32E-06 4.4E-09 3.97E-09 0 7.6E-11 1.71E-09 2.68E-11 -2.23E-03
ADPF MJ 2.13E+02 1.44E+01 5.64E-03 3.86E+00 2.67E-01 3.41E-01 0 3.59E-02 1.15E-01 3.91E-03 -4.11E+01
m3 world eq
WDP 2.58E+00 1.61E-03 2.21E-03 4.03E-02 3.32E-03 4.83E-03 0 4.97E-06 2.57E-02 3.13E-05 -5.84E-01
deprived
GWP = Global warming potential; ODP = Depletion potential of the stratospheric ozone layer; AP = Acidification potential of land and water; EP =
Eutrophication potential; POCP = Formation potential of tropospheric ozone photochemical oxidants; ADPE = Abiotic depletion potential for non-fossil
resources; ADPF = Abiotic depletion potential for fossil resources; WDP = Water (user) deprivation potential)
RESULTS OF THE LCA - INDICATORS TO DESCRIBE RESOURCE USE according to EN 15804+A2: 1 piece LA GARD 700
Parameter Unit A1-A3 A4 A5 B2 B6/1 B6/2 C1 C2 C3 C4 D
PERE MJ 3.03E+01 3.48E-02 1.52E-01 7.77E-01 1.19E-01 6.21E-02 0 1.13E-04 5.63E-02 5.13E-04 -5.3E+00
PERM MJ 1.77E-01 0 -1.51E-01 0 0 0 0 0 -2.64E-02 0 0
PERT MJ 3.06E+01 3.48E-02 1.02E-03 7.77E-01 1.19E-01 6.21E-02 0 1.13E-04 2.99E-02 5.13E-04 -5.3E+00
PENRE MJ 2.11E+02 1.44E+01 5.64E-03 3.86E+00 2.68E-01 3.42E-01 0 3.6E-02 3.54E+00 3.92E-03 -4.11E+01
PENRM MJ 3.43E+00 0 0 0 0 0 0 0 -3.43E+00 0 0
PENRT MJ 2.14E+02 1.44E+01 5.64E-03 3.86E+00 2.68E-01 3.42E-01 0 3.6E-02 1.15E-01 3.92E-03 -4.11E+01
SM kg 3.17E-02 0 0 0 0 0 0 0 0 0 0
RSF MJ 0 0 0 0 0 0 0 0 0 0 0
NRSF MJ 0 0 0 0 0 0 0 0 0 0 0
FW m3 7.56E-02 6.74E-05 5.21E-05 1.74E-03 1.37E-04 1.36E-04 0 2.03E-07 6.13E-04 9.87E-07 -1.72E-02
PERE = Use of renewable primary energy excluding renewable primary energy resources used as raw materials; PERM = Use of renewable primary
energy resources used as raw materials; PERT = Total use of renewable primary energy resources; PENRE = Use of non-renewable primary energy
excluding non-renewable primary energy resources used as raw materials; PENRM = Use of non-renewable primary energy resources used as raw
materials; PENRT = Total use of non-renewable primary energy resources; SM = Use of secondary material; RSF = Use of renewable secondary fuels;
NRSF = Use of non-renewable secondary fuels; FW = Use of net fresh water
RESULTS OF THE LCA – WASTE CATEGORIES AND OUTPUT FLOWS according to EN 15804+A2:
1 piece LA GARD 700
Parameter Unit A1-A3 A4 A5 B2 B6/1 B6/2 C1 C2 C3 C4 D
HWD kg 2.1E-06 1.38E-09 8.31E-12 4.84E-08 1.11E-10 1.34E-10 0 3.49E-12 4.37E-10 5.97E-11 -5.94E-07
NHWD kg 3.72E-01 1.46E-03 5.6E-04 7.27E-02 1.9E-04 1.18E-04 0 3.68E-06 2.57E-02 1.97E-02 4.19E-03
RWD kg 9.46E-03 1.18E-05 2.96E-07 8.97E-05 4.06E-05 2.77E-05 0 3.86E-08 4.3E-06 4.46E-08 -1.32E-03
CRU kg 0 0 0 0 0 0 0 0 0 0 0
MFR kg 0 0 0 0 0 0 0 0 4.87E-01 0 0
5 Environmental Product Declaration - dormakaba - LA GARD 700
MER kg 0 0 0 0 0 0 0 0 0 0 0
EEE MJ 2.47E-03 0 2.7E-02 0 0 0 0 0 0 0 0
EET MJ 4.47E-03 0 4.9E-02 0 0 0 0 0 0 0 0
HWD = Hazardous waste disposed; NHWD = Non-hazardous waste disposed; RWD = Radioactive waste disposed; CRU = Components for re-use;
MFR = Materials for recycling; MER = Materials for energy recovery; EEE = Exported electrical energy; EET = Exported thermal energy
RESULTS OF THE LCA – additional impact categories according to EN 15804+A2-optional:
1 piece LA GARD 700
Parameter Unit A1-A3 A4 A5 B2 B6/1 B6/2 C1 C2 C3 C4 D
Disease
PM 1.04E-06 1.4E-08 2.77E-11 9.82E-09 2.82E-10 7.54E-10 0 1.33E-11 5.64E-10 2.65E-11 -3.7E-07
incidence
IR kBq U235 eq 9.27E-01 1.61E-03 4.59E-05 8.82E-03 6.66E-03 2.62E-03 0 5.52E-06 3.9E-04 4.59E-06 -1.38E-01
ETP-fw CTUe 1.22E+02 1.02E+01 2.68E-03 1.32E+01 1.14E-01 9.86E-02 0 2.55E-02 4.33E-02 2.24E-03 -1.18E+01
HTP-c CTUh 5.31E-09 1.92E-10 1.42E-13 6.69E-11 3.16E-12 2.73E-12 0 4.79E-13 3.74E-12 3.31E-13 4.81E-09
HTP-nc CTUh 3.77E-07 8.85E-09 6.13E-12 7.74E-09 1.16E-10 1.07E-10 0 2.05E-11 3.77E-10 3.65E-11 5.76E-07
SQP SQP 5.05E+01 2.94E-02 1.5E-03 3.76E-01 8.52E-02 3.93E-02 0 9.24E-05 3.45E-02 8.16E-04 -2.57E+00
PM = Potential incidence of disease due to PM emissions; IR = Potential Human exposure efficiency relative to U235; ETP-fw = Potential comparative
Toxic Unit for ecosystems; HTP-c = Potential comparative Toxic Unit for humans (cancerogenic); HTP-nc = Potential comparative Toxic Unit for humans
(not cancerogenic); SQP = Potential soil quality index
Disclaimer 1 – for the indicator IRP
This impact category deals mainly with the eventual impact of low dose ionizing radiation on human health of the nuclear fuel cycle. It
does not consider effects due to possible nuclear accidents, occupational exposure nor radioactive waste disposal in underground
facilities. Potential ionizing radiation from the soil, from radon and from some construction materials is also not measured by this
indicator.
Disclaimer 2 – for the indicators ADPE, ADPF, WDP, ETP-fw, HTP-c, HTP-nc, SQP. The results of this environmental impact indicator
shall be used with care as the uncertainties on these results are high or as there is limited experienced with the indicator.
References
DIN EN 1300
DIN EN 1300:2019, Secure storage units - Classification for European Chemicals Agency
high security locks according to their resistance to unauthorized https://echa.europa.eu/de/
opening
Further References
DIN EN ISO 14025:
DIN EN ISO 14025:2011-10, Environmental labels and IBU 2021
declarations — Type III environmental declarations - Principles General Instructions for the EPD programme of Institut Bauen
and procedures. und Umwelt e.V. Version 2.0, Berlin: Institut Bauen und Umwelt
e.V., 2021. www.ibu-epd.com
EN 15804:2019+A2
EN 15804:2019+A2 (in press), Sustainability of construction GaBi ts software
works — Environmental Product Sphera Solutions GmbH
Declarations — Core rules for the product category of Gabi Software System and Database for Life Cycle
construction products. Engineering 1992-2020
Version 10.0.0.71
UL 2058 University of Stuttgart
UL 2058: 2005-06,Underwriters Laboratories, High-Security Leinfelden-Echterdingen
Electronic locks
GaBi ts documentation
VdS 2344 GaBi life cycle inventory data documentation
VdS 2344:2014-07, Procedure for the testing, approval and (https://www.gabi-software.com/support/gabi/gabidatabase-
certification of products and systems for fire protection and 2020-lci-documentation/).
security technologies
LCA-tool dormakaba
VdS 2396 LCA tool, version 1.0. SAL
VdS 2396:2014-07, VdS Guidelines for Physical Security Developed by Sphera Solutions GmbH.
Devices - High Security Locks for Secure Storage Units -
Requirements and Test Methods PCR Part A
PCR – Part A: Calculation Rules for the Life Cycle Assessment
(REACH) and Requirements on the Project Report according to EN
Regulation (EC) No 1907/2006 of the European Parliament and 15804+A2:2019, Version 1.0, Institut
of the Council on the Registration, Bauen und Umwelt e.V., www.ibu-epd.com.
Evaluation, Authorisation and Restriction of Chemicals
(REACH). PCR Part B
PCR – Part B: Requirements on the EPD for Electronic and
(RoHS) physical Access Control Systems, version 08/2021, Institut
Substances in electrical and electronic equipment (RoHS), Bauen und Umwelt e.V., www.ibu-epd.com.
Directive (EU) No 2011/65.
6 Environmental Product Declaration - dormakaba - LA GARD 700
Publisher
Institut Bauen und Umwelt e.V. +49 (0)30 3087748- 0
Hegelplatz 1 info@ibu-epd.com
10117 Berlin www.ibu-epd.com
Germany
Programme holder
Institut Bauen und Umwelt e.V. +49 (0)30 3087748- 0
Hegelplatz 1 info@ibu-epd.com
10117 Berlin www.ibu-epd.com
Germany
Author of the Life Cycle Assessment
Sphera Solutions GmbH +49 711 341817-0
Hauptstraße 111- 113 info@sphera.com
70771 Leinfelden-Echterdingen www.sphera.com
Germany
Owner of the Declaration
dormakaba International Holding GmbH +49 2333 793-0
DORMA Platz 1 info.de@dormakaba.com
58256 Ennepetal www.dormakaba.com
Germany
7 Environmental Product Declaration - dormakaba - LA GARD 700
