ENVIRONMENTAL PRODUCT DECLARATION
as per ISO 14025 and EN 15804+A2
Owner of the Declaration Give Steel A/S
Programme holder Institut Bauen und Umwelt e.V. (IBU)
Publisher Institut Bauen und Umwelt e.V. (IBU)
Declaration number EPD­GIV­20220233­IBA1­EN
Issue date 28.11.2022
Valid to 27.11.2027
Painted Structural Steel
Give Steel A/S
www.ibu-epd.com | https://epd-online.com
Umwelt Produktdeklaration Name des Herstellers – Name des Produkts
1. General Information
Give Steel A/S Painted Structural Steel
Programme holder Owner of the declaration
IBU – Institut Bauen und Umwelt e.V. Give Steel A/S
Hegelplatz 1 Sjællandsvej 14
10117 Berlin 7330 Brande
Germany
Declaration number Declared product / declared unit
EPD­GIV­20220233­IBA1­EN 1 t of painted structural steel.
This declaration is based on the product Scope:
category rules: The declaration covers painted structural steel
Structural steels, 11.2017 produced at the production site in Brande, Denmark.
(PCR checked and approved by the SVR) The declaration covers all life cycle modules from A1­
A5, C1­C4 and D and is based on product­specific data
provided by Give Steel A/S and background data from
Issue date
GaBi professional 2020 and Ecoinvent v3.6.
28.11.2022
The owner of the declaration shall be liable for the
Valid to
underlying information and evidence; the IBU shall not
27.11.2027
be liable with respect to manufacturer information, life
cycle assessment data and evidences.
The EPD was created according to the specifications
of EN 15804+A2. In the following, the standard will be
simplified as EN 15804.
Verification
The standard EN 15804 serves as the core PCR
Independent verification of the declaration and data
according to ISO 14025:2011
Dipl. Ing. Hans Peters internally x externally
(chairman of Institut Bauen und Umwelt e.V.)
Dr. Alexander Röder Mrs Kim Allbury
(Managing Director Institut Bauen und Umwelt e.V.)) (Independent verifier)
2. Product
2.1 Product description/Product definition structural steels – Part 1: General technical delivery
This EPD applies to 1 ton of painted structural steel. conditions and the CE­marking.
Structural steel constructions from Give Steel are 2.2 Application
designed and produced according to European design The product can be used as part elements or as an
codes and production standards, as well as in independent static system, where all parts are made of
compliance with project specifications. steel. The product is widely used in numerous
While Eurocode 1 and Eurocode 3 apply to the design construction projects. Examples are:
and civil engineering works, manufacturing is carried  Single­story buildings (industrial and storage
out according to EN 1090 for steel construction. halls, animal stables, data centres, etc.)
 Multi­story buildings (offices, residential
Furthermore, these codes and standards outline
buildings, car parks, etc.)
specific product standards for choosing the most
appropriate constitute products for each component.  Bridges (railway bridge, road bridge,
Such standards include EN 10025 which defines the pedestrian bridge, etc.)
requirements for non­alloy and fine grain weldable  Other structures (Stadiums, convention
structural steels, EN 10219 for cold formed hollow centres, airports, stations, etc.)
sections and EN 13479 and ISO 544 which sets out
the same set of requirements for materials.
For the placing on the market of the product in the 2.3 Technical Data
European Union/European Free Trade Association This EPD is valid for painted structural steel of different
(EU/EFTA) (with the exception of Switzerland) forms of delivery. Specific information on dimension
Regulation (EU) No. 305/2011 (CPR) applies. The tolerances, constructional data as well as mechanical
product needs a declaration of performance taking into and chemical properties can be found in the relevant
consideration EN 10025­1:2004 Hot rolled products of literature and/or the standards.
2 Environmental Product Declaration Give Steel A/S – Painted Structural Steel
are distributed for use as beams and to the welding
Constructional data robot, respectively. Beams and associated plates are
Name Value Unit stapled together. Beams are then welded, according to
Density 7850 kg/m3 design diagrams.
Modulus of elasticity 210000 N/mm2
Coefficient of thermal expansion 12 10­6K­1 When manufacturing welded wedges for robot welding,
Thermal conductivity 48 W/(mK) all parts are assembled from the CNC cutting table and
Melting point 1536 °C CNC flat iron cutter. Once the parts are collected they
are stapled together according to design diagrams.
The stapled wedges are robot welded and sent on.
Performance data of the product in accordance with The remaining components are mounted or welded
the declaration of performance with respect to its manually.
essential characteristics according to EN 10025, Hot
rolled products of structural steels. When the items are ready for surface treatment, they
are moved to the factory's painting booth, where they
2.4 Delivery status are painted according to the desired paint system,
The dimensions of the product declared in this EPD which is shown on a label on the beam. Drying follows
may vary depending on the intended application. the specifications of the paint supplier. Once dry, the
painted beams are ready for transportation to the
2.5 Base materials/Ancillary materials construction site.
The product constitutes primarily of steel scrap (78 %)
and primary steel (20 %). Welding rod (iron) and paint 2.7 Environment and health during
account for 1 % respectively. manufacturing
The painted structural steel does not contain During the entire manufacturing process, no other
substances listed in the ”Candidate List of Substances health protection measures are required
of Very High Concern for Authorisation” (SVHC). extending beyond the legally specified industrial
protection measures for commercial enterprises.
This product/article/at least one partial article contains
substances listed in the candidate list (date: 2.8 Product processing/Installation
08.08.2022) exceeding 0.1 percentage by mass: No The product is installed using a diesel truck. No
auxiliary materials are used.
This product/article/at least one partial article contains
other carcinogenic, mutagenic, reprotoxic (CMR) 2.9 Packaging
substances in categories 1A or 1B which are not on The product is delivered with metal strips and
the candidate list, exceeding 0.1 percentage by mass: cardboard as packaging.
No
Biocide products were added to this construction 2.10 Condition of use
product or it has been treated with biocide products During use, no changes in material composition shall
(this then concerns a treated product as defined by the occur. The product does not require maintenance.
(EU) Ordinance on Biocide Products No. 528/2012):
No 2.11 Environment and health during use
Under normal use conditions, structural steel products
2.6 Manufacture do not cause any adverse health effects nor release
The product stage comprises the acquisition of all raw other emissions to indoor air. Also, no environmental
materials, products and energy, transport to the impacts on water, air or soil are expected.
production site, packaging and waste processing up to
the ”end­of­waste” state or final disposal. The LCA 2.12 Reference service life
results are declared in aggregated form for the product A reference service life for structural steel is not
stage, which means. that the sub­modules A1, A2 and declared. It is a construction product with many
A3 are declared as one module A1­A3. different application purposes. The lifetime therefore
will be limited by the service life of the work.
The raw materials: flat iron, plate and beams are
brought in, processed, shot cleaned, cut and welded.
The process will vary, depending on the involved raw 2.13 Extraordinary effects
material.
Fire
The various materials are transported by side loader The material is class A1, i.e. not flammable per EN
from our warehouse to the appropriate production 13501. The material does not emit fumes or fire gases.
machines: Flat iron to the computerized numerical
control (CNC) flat iron machine, plate to the CNC Fire protection
plasma cutter and beams to the shot ball cleaner. Flat Name Value
iron is processed if necessary, by adding holes and Building material class according A1
cutting into strips. Plate is plasma cut following 2D to EN 13501­1
models. Beams are shot cleaned and cut to length.
Flat iron, steel plate and beams are shot cleaned Water
before production to produce the correct surface. The Steel is stable in water, insoluble and does not emit
shot cleaner is always kept full to save power. The substances in water. In case of flooding, no impacts
steel balls are reused in production until steel dust is are to be expected. Steel can corrode in the presence
all that remains. After cleaning, the flat iron and plate of oxygen in the water (= slow oxidation).
3 Environmental Product Declaration Give Steel A/S – Painted Structural Steel
Mechanical destruction cycle of reuse or recycling. However, in the case of
Steel components display very good characteristics dumping due to collection loss, no environmental
when exposed to extraordinary mechanical impact. As impacts are expected. Waste code in accordance with
a general rule, no chips, breaking edges or similar are the European Waste Catalogue (EWC): (17 04 05 Iron
incurred. and steel).
2.14 Re-use phase 2.16 Further information
The product has a 100 % recycling potential. Further information on the product can be obtained
from givesteel.com.
2.15 Disposal
Due to its high value as a resource, steel scrap is not
disposed of but instead fed into a well­established
3. LCA: Calculation rules
3.1 Declared Unit been omitted from the LCA study, as it is assumed to
The declared unit is 1 ton of painted structural steel. be negligible.
Thus, the declaration is in compliance with the rules in
The paint accounts for 1 % of the product's weight­%. EN 15804, 6.3.5, where the omission for input­flows
per module must be a maximum 5 % of energy usage
Declared unit and mass and at most 1 % for unit processes.
Name Value Unit
Declared unit 1 t 3.5 Background data
Density 7850 kg/m3 The LCA model is developed using GaBi Software
developed by Sphera Solutions GmbH. The
databases, GaBi Professional 2020 and EcoInvent 3.6,
provide the life cycle inventory data used from the
3.2 System boundary background system.
Type of EPD: Cradle to gate with options.
Module A1­A3, A4, A5, B1­B7, C1­C4 and D are 3.6 Data quality
considered. Yet, no environmental impacts are The product­specific data have been collected by Give
associated with modules B1­B7, thus, these modules Steel A/S and are based on the yearly production
are declared as 'not relevant'. amounts and energy consumption at the production
site located in Brande, Denmark in 2019. Background
Modules A1-A3 include the acquisition of all raw data are based on GaBi Professional and EcoInvent
materials, products and energy, transport to the 3.6 and are less than 10 years old. Generally, the used
production site, the manufacturing of the painted background datasets are of good quality, and the
structural steel and waste processing up to the ”end­of­ majority of the datasets are only a couple of years old.
waste” state.
3.7 Period under review
Module A4 includes the transport of the product to the The foreground data was collected by Give Steel A/S
construction site. in the period January 2019 to December 2019. The
Module A5 includes the installation of the product declaration is therefore based on average values for
using a diesel truck. the production amount from the year 2019.
Module C1 considers the deconstruction of the 3.8 Allocation
structural steel using a truck. In module C2, the The allocation is made in accordance with the
demolished steel is transported to a waste processing provisions of EN 15804. A conservative approach is
site, with the waste processing considered in module used for the allocation of by­products in steel
C3. manufacturing, meaning that all impact is attributed to
the main product of steel. Energy, heat and water
Finally, module D considers the benefits from consumption at the production site is allocated through
recycling the demolished steel parts. mass allocation.
3.3 Estimates and assumptions 3.9 Comparability
It is assumed that 100 % of the product can be Basically, a comparison or an evaluation of EPD data
recycled, though 5 % of the product is lost at recycling. is only possible if all the data sets to be compared
The recycling of the product is assumed to replace were created according to EN 15804 and the building
scrap steel in module D. context, respectively the product­specific
characteristics of performance, are taken into account.
3.4 Cut-off criteria
The declaration covers all relevant processes and Background information was mainly taken from GaBi
aspects of the life cycle for painted structural steel. Professional 2020. Ecoinvent 3.6 was used when
Only the production of capital goods, buildings and datasets where not available in GaBi Professional
equipment during the production of steel in A1 has 2020.
4. LCA: Scenarios and additional technical information
Characteristic product properties
4 Environmental Product Declaration Give Steel A/S – Painted Structural Steel
Information on biogenic Carbon
The product does not contain any biogenic carbon.
The packaging includes a small amount of biogenic
carbon, as cardboard is used as packaging.
Note: 1 kg biogenic carbon is equivalent to 44/12 kg of
CO
2
Information on describing the biogenic Carbon
Content at factory gate
Name Value Unit
Biogenic Carbon Content in
0 kg C
product 0
Biogenic Carbon Content in
0.012 kg C
accompanying packaging 0
Transport to the building site (A4)
Name Value Unit
Litres of fuel 2.7 l/100km
Transport distance 300 km
Capacity utilisation (including
85 %
empty runs)
Gross density of products
7850 kg/m3
transported
Capacity utilisation volume factor 0.55 ­
Installation into the building (A5)
A diesel truck is used to install the product. Based on
annual data from Give Steel A/S, 0.261 kg diesel is
used for the installation of 1 ton of structural steel.
Name Value Unit
Other resources Diesel 0.261 kg
Use stage (B1-B7)
There are no environmental impacts associated with
the use stage (B1­B7).
Reference service life
The reference service life of the product depends on its
application.
End of life (C1 - C4)
Name Value Unit
Collected separately structural
1000 kg
steel
Collected as mixed construction
0 kg
waste
Reuse 0 kg
Recycling 980 kg
Energy recovery 10 kg
Landfilling 0 kg
Reuse, recovery and/or recycling potentials (D),
relevant scenario information
The product has a 100 % recycling potential, yet, 5 %
of the product is assumed to be lost through the
recycling process.
5 Environmental Product Declaration Give Steel A/S – Painted Structural Steel
5. LCA: Results
The LCA results cover modules A1­A5, C1­C4 and D. No environmental impacts are associated with modules B1­
B7; thus, these modules are marked as 'not relevant' or 'not declared' in the table below.
DESCRIPTION OF THE SYSTEM BOUNDARY (X = INCLUDED IN LCA; ND = MODULE OR INDICATOR NOT
DECLARED; MNR = MODULE NOT RELEVANT)
BENEFITS AND
CONSTRUCTI LOADS
PRODUCT STAGE ON PROCESS USE STAGE END OF LIFE STAGE BEYOND THE
STAGE SYSTEM
BOUNDARIES
6 Environmental Product Declaration Give Steel A/S – Painted Structural Steel
lairetam
waR
ylppus tropsnarT
gnirutcafunaM
eht
morf
tropsnarT
etis
eht
ot
etag
ylbmessA esU
ecnanetniaM
riapeR
tnemecalpeR tnemhsibrufeR
ygrene
lanoitarepO esu
retaw
lanoitarepO esu
noitcurtsnoc­eD
noitilomed tropsnarT
gnissecorp
etsaW
lasopsiD ­esueR ­yrevoceR ­gnilcyceR laitnetop
A1 A2 A3 A4 A5 B1 B2 B3 B4 B5 B6 B7 C1 C2 C3 C4 D
X X X X X ND ND MNR MNR MNR ND ND X X X X X
RESULTS OF THE LCA - ENVIRONMENTAL IMPACT according to EN 15804+A2: 1 ton painted structural
steel
Core Indicator Unit A1-A3 A4 A5 C1 C2 C3 C4 D
GWP­total [kg CO2­Eq.] 1.05E+3 8.39E+0 6.58E­1 6.58E­1 8.47E+0 4.23E+1 0.00E+0 ­3.18E+2
GWP­fossil [kg CO2­Eq.] 1.05E+3 8.23E+0 6.93E­1 6.93E­1 8.32E+0 4.36E+1 0.00E+0 ­3.18E+2
GWP­biogenic [kg CO2­Eq.] 1.11E+0 8.95E­2 0.00E+0 0.00E+0 9.04E­2 ­8.76E­4 0.00E+0 ­1.67E­1
GWP­luluc [kg CO2­Eq.] 1.27E+0 6.74E­2 7.62E­3 7.62E­3 6.80E­2 2.87E­2 0.00E+0 4.14E­2
ODP [kg CFC11­Eq.] 8.47E­12 1.53E­15 1.73E­16 1.73E­16 1.54E­15 3.54E­6 0.00E+0 ­5.57E­13
AP [mol H+­Eq.] 3.01E+0 3.00E­2 3.41E­3 3.41E­3 3.03E­2 3.09E­1 0.00E+0 ­5.71E­1
EP­freshwater [kg P­Eq.] 1.69E­3 2.54E­5 2.87E­6 2.87E­6 2.56E­5 2.09E­2 0.00E+0 ­7.67E­5
EP­marine [kg N­Eq.] 8.52E­1 1.37E­2 1.52E­3 1.52E­3 1.38E­2 7.17E­2 0.00E+0 ­8.59E­2
EP­terrestrial [mol N­Eq.] 9.25E+0 1.53E­1 1.69E­2 1.69E­2 1.54E­1 8.10E­1 0.00E+0 ­8.39E­1
POCP [kg NMVOC­Eq.] 2.63E+0 2.67E­2 4.29E­3 4.29E­3 2.70E­2 2.19E­1 0.00E+0 ­4.36E­1
ADPE [kg Sb­Eq.] 1.46E­4 6.73E­7 7.61E­8 7.61E­8 6.80E­7 1.37E­3 0.00E+0 ­6.87E­4
ADPF [MJ] 1.18E+4 1.11E+2 1.26E+1 1.26E+1 1.12E+2 3.79E+2 0.00E+0 ­2.78E+3
[m³ world­Eq
WDP ­3.12E+1 8.12E­2 9.18E­3 9.18E­3 8.20E­2 9.34E+0 0.00E+0 ­6.21E+1
deprived]
GWP = Global warming potential; ODP = Depletion potential of the stratospheric ozone layer; AP = Acidification potential of land and water; EP =
Caption Eutrophication potential; POCP = Formation potential of tropospheric ozone photochemical oxidants; ADPE = Abiotic depletion potential for non­
fossil resources; ADPF = Abiotic depletion potential for fossil resources; WDP = Water (user) deprivation potential
RESULTS OF THE LCA - INDICATORS TO DESCRIBE RESOURCE USE according to EN 15804+A2: 1 ton
painted structural steel
Indicator Unit A1-A3 A4 A5 C1 C2 C3 C4 D
PERE [MJ] 2.18E+3 6.42E+0 7.26E­1 7.26E­1 6.49E+0 5.52E+1 0.00E+0 2.25E+2
PERM [MJ] 5.88E­2 0.00E+0 0.00E+0 0.00E+0 0.00E+0 0.00E+0 0.00E+0 0.00E+0
PERT [MJ] 2.18E+3 6.42E+0 7.26E­1 7.26E­1 6.49E+0 5.52E+1 0.00E+0 2.25E+2
PENRE [MJ] 1.18E+4 1.11E+2 1.26E+1 1.26E+1 1.13E+2 3.79E+2 0.00E+0 ­2.78E+3
PENRM [MJ] 0.00E+0 0.00E+0 0.00E+0 0.00E+0 0.00E+0 0.00E+0 0.00E+0 0.00E+0
PENRT [MJ] 1.18E+4 1.11E+2 1.26E+1 1.26E+1 1.13E+2 3.79E+2 0.00E+0 ­2.78E+3
SM [kg] 7.84E+2 0.00E+0 0.00E+0 0.00E+0 0.00E+0 0.00E+0 0.00E+0 0.00E+0
RSF [MJ] 0.00E+0 0.00E+0 0.00E+0 0.00E+0 0.00E+0 0.00E+0 0.00E+0 0.00E+0
NRSF [MJ] 0.00E+0 0.00E+0 0.00E+0 0.00E+0 0.00E+0 0.00E+0 0.00E+0 0.00E+0
FW [m³] 2.05E+0 7.48E­3 8.46E­4 8.46E­4 7.56E­3 2.18E­1 0.00E+0 ­1.40E+0
PERE = Use of renewable primary energy excluding renewable primary energy resources used as raw materials; PERM = Use of
renewable primary energy resources used as raw materials; PERT = Total use of renewable primary energy resources; PENRE = Use of
non­renewable primary energy excluding non­renewable primary energy resources used as raw materials; PENRM = Use of non­
Caption
renewable primary energy resources used as raw materials; PENRT = Total use of non­renewable primary energy resources; SM = Use
of secondary material; RSF = Use of renewable secondary fuels; NRSF = Use of non­renewable secondary fuels; FW = Use of net fresh
water
RESULTS OF THE LCA – WASTE CATEGORIES AND OUTPUT FLOWS according to EN 15804+A2:
1 ton painted structural steel
Indicator Unit A1-A3 A4 A5 C1 C2 C3 C4 D
HWD [kg] 9.64E­5 5.16E­6 5.83E­7 5.83E­7 5.21E­6 3.32E­8 0.00E+0 7.21E­7
NHWD [kg] 1.15E+1 1.77E­2 2.00E­3 2.00E­3 1.78E­2 2.59E+0 0.00E+0 3.29E+1
RWD [kg] 3.03E­1 2.06E­4 2.32E­5 2.32E­5 2.08E­4 3.95E­4 0.00E+0 ­6.71E­4
CRU [kg] 0.00E+0 0.00E+0 0.00E+0 0.00E+0 0.00E+0 0.00E+0 0.00E+0 0.00E+0
MFR [kg] 0.00E+0 0.00E+0 0.00E+0 0.00E+0 0.00E+0 1.86E+2 0.00E+0 0.00E+0
MER [kg] 6.19E+0 0.00E+0 0.00E+0 0.00E+0 0.00E+0 1.00E+1 0.00E+0 0.00E+0
EEE [MJ] 0.00E+0 0.00E+0 0.00E+0 0.00E+0 0.00E+0 0.00E+0 0.00E+0 0.00E+0
EET [MJ] 0.00E+0 0.00E+0 0.00E+0 0.00E+0 0.00E+0 0.00E+0 0.00E+0 0.00E+0
HWD = Hazardous waste disposed; NHWD = Non­hazardous waste disposed; RWD = Radioactive waste disposed; CRU = Components
Caption for re­use; MFR = Materials for recycling; MER = Materials for energy recovery; EEE = Exported electrical energy; EET = Exported
thermal energy
RESULTS OF THE LCA – additional impact categories according to EN 15804+A2-optional:
1 ton painted structural steel
Indicator Unit A1-A3 A4 A5 C1 C2 C3 C4 D
[Disease
PM 3.75E­5 1.72E­7 3.76E­8 3.76E­8 1.74E­7 3.85E­6 0.00E+0 ­9.59E­6
Incidence]
[kBq U235­
IRP 2.79E+1 3.03E­2 3.43E­3 3.43E­3 3.06E­2 3.58E+0 0.00E+0 8.20E+0
Eq.]
ETP­fw [CTUe] 3.12E+3 8.31E+1 9.40E+0 9.40E+0 8.39E+1 1.70E+3 0.00E+0 ­4.16E+0
HTP­c [CTUh] 7.51E­7 1.72E­9 1.94E­10 1.94E­10 1.73E­9 3.65E­8 0.00E+0 1.06E­7
HTP­nc [CTUh] 1.85E­5 1.00E­7 1.08E­8 1.08E­8 1.01E­7 1.74E­6 0.00E+0 ­4.31E­6
SQP [­] 2.27E+3 3.90E+1 4.41E+0 4.41E+0 3.94E+1 7.00E+2 0.00E+0 5.99E+1
PM = Potential incidence of disease due to PM emissions; IR = Potential Human exposure efficiency relative to U235; ETP­fw = Potential
Caption comparative Toxic Unit for ecosystems; HTP­c = Potential comparative Toxic Unit for humans (cancerogenic); HTP­nc = Potential
comparative Toxic Unit for humans (not cancerogenic); SQP = Potential soil quality index
Disclaimer 1 – for the indicator “Potential Human exposure efficiency relative to U235”.
This impact category deals mainly with the eventual impact of low dose ionizing
radiation on human health of the nuclear fuel cycle. It does not consider effects due to possible
nuclear accidents, occupational exposure nor due to radioactive waste disposal in underground
facilities. Potential ionizing radiation from the soil, from radon and from some construction materials is also not
measured by this indicator.
Disclaimer 2 – for the indicators “abiotic depletion potential for non­fossil resources”, “abiotic depletion potential
for fossil resources”, “water (user) deprivation potential, deprivation­weighted water consumption”, “potential
comparative toxic unit for ecosystems”, “potential comparative toxic unit for humans – cancerogenic”, “Potential
comparative toxic unit for humans ­ not cancerogenic”, “potential soil quality index”.
The results of this environmental impact indicator shall be used with care as the
uncertainties on these results are high or as there is limited experienced with the indicator.
6. LCA: Interpretation
The calculated environmental impacts primarily stem includes both the production of scrap steel and ore­
from the production of scrap steel, which accounts for based steel.
78 % of the product's weight. The production of scrap The structural steel product is manufactured using
steel is the main contributor to 6 out of 19 water, electricity and heat at the production site in
environmental impact categories. The production of Brande, Denmark. These processes only have a minor
ore­based steel is the main contributor to 8 out of 19 effect on the overall environmental impacts of the
environmental impact categories. The most dominant product. The main contributor to the environmental
module is therefore module A1, since the module impacts in module A3 is heat consumption, as natural
gas is used.
7. Requisite evidence
concentrations in toluene equivalents according to EN
7.1 Corrosion 16516. All test results are calculated as specific
Paint and thickness of the layer are determined in emission rates, and as extrapolated air concentrations
accordance with EN ISO 12944-6:2018 which also in the European Reference Room (EN 16516, AgBB,
considers the expected lifetime of the product. EMICODE, M1 and Indoor Air Comfort).
7.2 VOC emissions AgBB overview of results (28 days [μg/m3])
Testing for VOC emissions has been conducted in Name Value Unit
accordance with EN ISO 16000-6. TVOC 110 μg/m3
Analysis of the air sampled on Tenax was performed at TSVOC <5 μg/m3
Eurofins Product Testing A/S under DANAK VOC without NIK/LCI <5 μg/m3
accreditation 392. Report no. 392­2021­ Carcinogenic Substances <1 μg/m3
00087505_A_EN. Reporting of measured
8. References
Standards EN 1090­2:2018, Execution of steel structures and
aluminium structures ­ Part 2: Technical requirements
AgBB for steel structures.
AgBB, Ausschuss zur gesundheitlichen Bewertung von
Bauprodukten (Committee for Health­related EN 10025
Evaluation of Building Products). EN 10025­2:2019, Hot rolled products of structural
steels ­ Part 2: Technical delivery conditions for non­
EN 1090 alloy structural steels.
EN 10219
7 Environmental Product Declaration Give Steel A/S – Painted Structural Steel
EN 10219­1:2006, Cold formed welded structural CPR
hollow sections of non­alloy and fine grain steels ­ Part Regulation (EU) No 305/2011 of the European
1: Technical delivery conditions. Parliament and of the Council of 9 March 2011 laying
down harmonised conditions for the marketing of
EN 13479 construction products and repealing Council Directive
EN 13479:2017, Welding consumables ­ General 89/106/EEC Text with EEA relevance.
product standard for filler metals and fluxes for fusion
welding of metallic materials. EMICODE
https://www.emicode.com/
EN 13501
EN 13501­1:2010, Fire classification of construction Eurofins Product Testing
products and building elements. https://www.eurofins.dk/product­testing/
EN 15804 EWC
EN 15804:2012+A2:2019+AC:2021, Sustainability of European Waste Catalogue, European Commission
construction works — Environmental Product
Declarations — Core rules for the product category of PCR Part A
construction products. Calculation Rules for the Life Cycle Assessment and
Requirements on the Project Report according to EN
EN 16516 15804+A2:2019. Institut Bauen und Umwelt e.V. (IBU).
EN 16516:2017+A1:2020, Construction products: Version 1.2. November 2021. www.ibu­epd.com
Assessment of release of dangerous substances.
Determination of emissions into indoor air. PCR Part B
Requirements on the EPD for www.ibu­epd.com
ISO 544 Structural steels. Institut Bauen und Umwelt e.V. (IBU).
ISO 544:2017, Welding consumables — Technical Version 1.1. 2017. www.ibu­epd.com
delivery conditions for filler materials and fluxes —
Type of product, dimensions, tolerances and markings. Software
ISO 12944 GaBi Software
ISO 12944­6:2018, Paints and varnishes — Corrosion Sphera Solutions GmbH. (2020). For further
protection of steel structures by protective paint information see: gabi.sphera.com/international/index
systems — Part 6: Laboratory performance test
methods. Databases
ISO 14025 GaBi Professional
ISO 14025:2011, Environmental labels and Sphera Solutions GmbH. (2020). GaBi LCA Database
declarations — Type III environmental declarations — Documentation. Retrieved from
Principles and procedures. gabi.sphera.com/international/support/gabi
ISO 16000-6 EcoInvent 3.6
ISO 16000­6:2011, Indoor air ­ Part 6: Determination of http://www.gabi­software.com/nw­eu­
volatile organic compounds in indoor and test chamber danish/databases/ecoinvent
air by active sampling on Tenax TA sorbent, thermal
desorption and gas chromatography using MS or IBU 2021
MSFID. Institut Bauen und Umwelt e.V.: General Instructions
for the EPD programme of Institut Bauen und Umwelt
Further references e.V., Version 2.0, Berlin: Institut Bauen und Umwelt
e.V., 2021
Candidate List of Substances of Very High www.ibu­epd.com
Concern for Authorisation
Candidate List of substances of very high concern for
Authorisation, 2021, ECHA, echa.europa.eu .
8 Environmental Product Declaration Give Steel A/S – Painted Structural Steel
Publisher
Institut Bauen und Umwelt e.V. Tel +49 (0)30 3087748­ 0
Hegelplatz 1 Fax +49 (0)30 3087748­ 29
10117 Berlin Mail info@ibu­epd.com
Germany Web www.ibu-epd.com
Programme holder
Institut Bauen und Umwelt e.V. Tel +49 (0)30 ­ 3087748­ 0
Hegelplatz 1 Fax +49 (0)30 – 3087748 ­ 29
10117 Berlin Mail info@ibu­epd.com
Germany Web www.ibu-epd.com
Author of the Life Cycle
Assessment Tel 56 40 00 00
COWI A/S Fax ­
Parallelvej 2 Mail cowi@cowi.com
2800 Kgs. Lyngby Web https://www.cowi.com/
Denmark
Owner of the Declaration
Give Steel A/S Tel +4575731218
Sjællandsvej 14 Fax +4575731275
7330 Brande Mail info@givesteel.com
Denmark Web givesteel.com
