ENVIRONMENTAL PRODUCT DECLARATION
as per ISO 14025 and EN 15804+A2
Owner of the Declaration Grundfos Holding A/S
Publisher Institut Bauen und Umwelt e.V. (IBU)
Programme holder Institut Bauen und Umwelt e.V. (IBU)
Declaration number EPD-GRU-20230075-CBC1-EN
Issue date 21.11.2023
Valid to 20.11.2028
MAGNA3 100-80/100/120 (Cast Iron)
Grundfos Holding A/S
www.ibu-epd.com | https://epd-online.com
General Information
Grundfos Holding A/S MAGNA3 100-80/100/120 (Cast Iron)
Programme holder Owner of the declaration
IBU – Institut Bauen und Umwelt e.V. Grundfos Holding A/S
Hegelplatz 1 Poul Due Jensens Vej 7
10117 Berlin 8850 Bjerringbro
Germany Denmark
Declaration number Declared product / declared unit
EPD-GRU-20230075-CBC1-EN 1 PCS. of MAGNA3 100-80/100/120 (Cast Iron)
This declaration is based on the product category rules: Scope:
Pumps for liquids and liquids with solids, 01.08.2021 The declaration applies to 1 piece of MAGNA3 (Cast Iron) pump.
(PCR checked and approved by the SVR) The product is produced in Wahlstedt, Germany, and the life cycle
assessment is based on data collected at the production site.
Issue date Production has been modeled using annual production data from 2021.
The declaration covers three different types of the MAGNA3 100- product
21.11.2023
(80/100/120).
The owner of the declaration shall be liable for the underlying information
and evidence; the IBU shall not be liable with respect to manufacturer
Valid to
information, life cycle assessment data and evidences.
20.11.2028
The EPD was created according to the specifications of EN 15804+A2. In
the following, the standard will be simplified as EN 15804.
Verification
The standard EN 15804 serves as the core PCR
Independent verification of the declaration and data according to ISO
14025:2011
internally X externally
Dipl.-Ing. Hans Peters
(Chairman of Institut Bauen und Umwelt e.V.)
Florian Pronold Mrs Kim Allbury,
(Managing Director Institut Bauen und Umwelt e.V.) (Independent verifier)
1 Environmental Product Declaration - Grundfos Holding A/S - MAGNA3 100-80/100/120 (Cast Iron)
Product
Standards used:
Product description/Product definition EN 16297-1:2012, EN 16297-2:2012, EN 16297-3:2012.
The Grundfos MAGNA3 circulator pumps are designed for
circulating liquids in heating systems, air conditioning and The CE marking takes into account the proof of conformity with
cooling systems and domestic hot water systems. However, the the respective harmonized norms based on the legal provisions
pump range can also be used in ground source heat pump above.
systems and solar heating systems.
MAGNA3 pumps are not harmonized in accordance with the
The MAGNA3 pump is a centrifugal pump powered by an CPR.
electrical motor. It has a high-performance neodymium magnet
rotor which increases motor efficiency and an insulation shell to Application
reduce heat loss from the cast iron pump housing with threaded For the application and use the respective national provisions
connections. apply.
The declaration covers three types of the MAGNA3 pump. They
are grouped as shown below. The group reference in the The pump is designed for circulating liquids in the following
technical data and scenarios refers also to these. systems:
GROUP 1 - MAGNA3 100-80 · heating systems
GROUP 2 - MAGNA3 100-100 GROUP 3 - MAGNA 3 100-120 · domestic hot-water systems
· air-conditioning and cooling systems
These are all the same physical products and 100 % identical · ground-source heat-pump systems
in terms of design, dimensions and materials as well as supply · solar-heating systems
chain and manufacturing processes, i.e., all cradle to gate
processes (A1-A3). The pump is suitable for thin, clean, non-aggressive and non-
explosive liquids, not containing solid particles or fibres that
The products are also identical in terms of packaging, may attack the pump mechanically or chemically. In heating
distribution, reference service life and end-of-life treatment. systems, the water must meet the requirements of accepted
standards on water quality in heating systems. The pumps are
The only thing that differentiates the products from each other also suitable for domestic hot-water systems
is the software which controls how the pump operates in the
system in which it is installed, making them fit for different Technical Data
applications. Hence, all life cycle modules are identical, except The performance data of the product according to the
use stage module B6, which will change, as the applied harmonized norms, based on the harmonization provisions
scenarios for electricity consumption changes. For the placing above apply.
on the market in the European Union/European Free Trade The relevant technical specifications according to the PCR Part
Association (EU/EFTA) (with the exception of Switzerland) the B are given in the table below.
following legal provisions apply: Characteristics that are the same for all product groups are only
given once. Others are given individually for all three groups.
Machinery Directive (2006/42/EC) Constructional data
Standard used: EN 809:1998 + A1:2009.
Name Value Unit
Frequency 50 Hz
Radio Equipment Directive (2014/53/EU)
Standards used: Voltage 230 V
EN 60335-1:2012/AC:2014 + A11:2014, EN 60335-2-51:2003 + Clean
Pumped liquid (e.g. water) -
A1:2008 + A2:2012, EN 62233:2008. Water
Energy Efficiency Index Gr.1 0,17
EN 55014-1:2006 + A1:2009 + A2:2011, EN 55014-1:2017, EN
Energy Efficiency Index Gr.2 0,17
61000-6-2:2005, EN 61000-3-2:2014, EN 61000-3-3:2013,
Energy Efficiency Index Gr.3 0,17
ETSI EN 301 489-1 V2.2.0, ETSI EN 301 489-17 V3.2.0. ETSI
EN 300 328 V2.1.1 Flow range Gr. 1 (max) 60,0 m3/h
Flow range Gr. 2 (max) 66,0 m3/h
Electromagnetic Compatibility (EMC) Directive Flow range Gr. 3 (max) 71,0 m3/h
(2014/30/EU)
Head max. Gr.1 8 m
Standards used:
Head max. Gr.2 10 m
EN 55014-1:2017, EN 55014-2:2015,
Head max. Gr.3 12 m
EN 61000-3-2:2014/2019, EN 61000-6-2:2008/2019, Power input Gr. 1 Average (from load profile
0,404 kW
describing use)
EN 61000-3-3:2013 A1:2019 Power input Gr. 2 Average (from load profile
0,558 kW
describing use)
RoHS Directive 2011/65/EU and 2015/863//EU
Power input Gr. 3 Average (from load profile
Standard: EN 50581:2012. 0,636 kW
describing use)
Nominal capacity Gr.1 0,95 kW
Ecodesign Directive (2009/125/EC)
Commission Regulation (EC) No: 641/2009 and Commission Nominal capacity Gr. 2 1,21 kW
Regulation (EU) 622/2012 Nominal capacity Gr.3 1,54 kW
2 Environmental Product Declaration - Grundfos Holding A/S - MAGNA3 100-80/100/120 (Cast Iron)
Performance data of the product according to the harmonized 10.06.2022) exceeding 0.1 percentage by mass: no
standards, based on provisions for harmonization.
The Wahlstedt production has been assessed and certified as
Base materials/Ancillary materials meeting the requirements in ISO 14001, ISO 50001, ISO 45001
Base materials / Ancillary materials and ISO 9001
Name Value Unit Reference service life
Aluminium 10 % No use stage scenario which refers to the lifetime of the product
Cast iron 60 % is declared. However, to facilitate building calculations, an
Ceramics 0,2 % estimated RSL of 10 years can be used.
This is an EU consensus-based estimation, referenced on page
Copper 3 %
37 in Appendix 7: Lot 11 – Circulators in Buildings, prepared by
Electronics 0,2 %
AEA Energy & Environment for the European Commission in
Magnet Nd 1 % the context of the Eco Design Directive:
Paper 0,3 %
PCB 2 % There is no definitive information on the average circulator life
available, there is consensus within the industry that it is at
Plastics 0,2 %
least 12 years. However, this is complicated by many factors,
Plastics, foam 1 %
including many being scrapped prematurely when e.g. the
Plastics GF 3 % boiler they are connected to is replaced.
Rubber 0,1 %
Stainless steel 3 % From the estimated stock (140Mpa) and annual sales (14Mpa),
Steel 8 % the average lifetime of the circulator is taken as 10 years for the
purposes of this study.
Cardboard 7 %
Plastic film 0,04 %
The RSL of the declared product is not directly influencing the
TOTAL 100 % results in this study, as no declared use stage scenario is
dependent on the RSL; The use stage sub-module B6 is
REACH
declared per year as required by the PCR Part B.
This product/article/at least one partial article contains
substances listed in the ECHA candidate list (date:
LCA: Calculation rules
system and the following manufacturing, transport up to the
Declared Unit factory gate as well as the processing any waste arising from
The declared unit is 1 piece (pcs.) of MAGNA3 (Cast Iron) those processes.
pump. Wastes and losses are included in the modules where they
Name Value Unit occur according to the polluter pays principle and the modular
Declared unit 1 pce. approach of EN 15804.
Mass reference 37.23 kg/pce
The product includes:
Conversion factor [Mass/Declared Unit] 37.23
For IBU core EPDs (where clause 3.6 is part of the EPD): for · A1 Extraction and processing of raw materials;
average EPDs, an estimate of the robustness of the LCA · A1 Reuse of products or materials from a previous product
values must be made, e.g. concerning the variability of the system;
production process, geographical representativeness and the · A1 Processing of secondary materials;
influence of background data and preliminary products · A1 Generation of electricity, steam and heat from primary
compared to the environmental impacts caused by the actual energy resources, also including their extraction, refining and
production. transport;
· A1 Energy recovery and other recovery processes from
secondary fuels;
System boundary
· A2 Transportation up to the factory gate and internal transport;
This EPD is Cradle-To-Grave. The system boundaries of the · A3 Production of ancillary materials or pre products;
EPD follow the modular approach in EN 15804. By decision no. · A3 Manufacturing of products and coproducts;
20170712-n of the SVR, the modules B3, B4 and B5 are by · A3 Manufacturing of packaging;
default declared as "MNR" (module not relevant). · A1-A3 processing up to the end-of-waste state or disposal of
final residues.
The product stage (A1-A3) comprises raw material extraction
and processing, transport processes as well as the For secondary material inputs, the system boundary to the
manufacturing process. The final production and assembly of previous system (providing the secondary material) is set where
the MAGNA3 pump takes place at a Grundfos manufacturing outputs reach the end-of-waste state. The recycling of
site in Germany. However, the full supply-chain leading to the secondary material into new raw materials is included in the
finished product at the gate is rather complex and includes a system boundary of this study. Waste materials from production
large amount of raw materials, components and semi-finished processes that is recycled without any modification of the
parts which comes from both external suppliers as well as other material inherent characteristics are modelled as closed loop
Grundfos production facilities. within A1-A3. This is done up to the input mass flow that was
used during production.
The product stage is included in the study, and according to EN
15804 the system boundary with nature is set to include those Waste for incineration arising in the product stage is accounted
processes that provide the material and energy inputs into the
3 Environmental Product Declaration - Grundfos Holding A/S - MAGNA3 100-80/100/120 (Cast Iron)
for in the module where the waste is produced. The (B6) come from the electricity consumption of the product. The
environmental loads from the incineration process are declared annual electricity consumption is calculated by multiplying the
in the module where it occurs and the electricity and heat which average power input, which is based on a defined load profile,
is produced from the incineration are considered as closed-loop with the annual running hours. For use stage (B6) European
within A1-A3, as described in PCR Part A, 5.5.1. The input of Average electricity grid mix has been used. These values are
biogenic carbon from the production of packaging material is declared in the scenarios section.
inventoried in A3. As required by PCR Part A, the
corresponding end-of-life module of the packaging material, A5, The End-of-Life stage (C1-C4) includes all activities from
is also declared and the emissions of biogenic carbon are when the product reaches the end of its service life and no
inventoried. longer provides any functionality and until all materials and
components are processed for reuse/recycling or disposed of.
The construction process stage (A4-A5) includes:
According to EN 15804 and the PCR Part A, the end-of-life
A4: stage includes:
· Transportation from factory gate to distribution center: · C1 deconstruction of the product from the building, including
· Consumption of electricity, thermal energy and water at initial on-site sorting of the materials;
distribution center; · C2 transportation of the discarded product to a recycling site
· Transportation from distribution center to construction site; and transportation of waste to final disposal;
· Wastage during distribution. · C3 waste processing, collection of waste fractions from the
deconstruction and waste processing of material flows intended
A5: for reuse, recycling and energy recovery;
· Installation process; · C4 waste disposal including physical pretreatment and
· Transport of packaging waste to treatment site; management of the disposal site.
· Waste treatment of packaging.
At the end of life, the MAGNA3 pump is manually disassembled
The packaging material does not reach the end of waste state from the piping system in which it has been installed. The
but is incinerated as waste. definition of the applied end-of-life scenario in this EPD follows
According to European statistics, the average R1 value of the requirements in the
incineration plants is > 0.6. Therefore, it is assumed
PCR Part A, 6.2 regarding complex products, with a
that packaging material is treated thermally in an incineration combination of recycling, thermal waste treatment and
plant with R1 > 0.6. The loads from the combustion process of landfilling. 100 % of the material is considered in the end-of-life
packaging are declared in module A5 and the resulting energy scenario as required by the PCR. An overall collection rate of
benefits in module D, as required by the PCR Part A, 5.5.2. 90 % has been assumed.
Use stage (B1-B7): Materials from which energy is recovered in an incineration
process with an R1-value above 0.60 are in this study included
The use stage, related to the building fabric includes: with the environmental burdens from the incineration process
inventoried in C3, the recovered energy is declared as exported
· B1, use or application of the installed product; energy in C3 and the energy benefits are declared in D. This
· B2, maintenance. procedure is according to the PCR Part A, 5.5.6. C3 includes
the mechanical separation of the product followed by a series
The use stage related to the operation of the building includes: of sorting steps. Metal fractions are recycled and plastics,
cardboard and electronics are assumed incinerated with energy
· B6, operational energy use; recovery. The residual fractions are landfilled and declared in
· B7, operational water use. C4.
In this study, all use stage modules are assessed, though B1, The specific amounts are shown in the scenarios section.
B2 and B7 are assessed to be zero. By decision no. 20170712-
n of the SVR, the modules B3, B4 and B5 are by default Beyond system boundary (D): According to EN 15804
declared as "MNR" (module not relevant). module D includes the reuse, recovery and/or recycling
The modules include the provision and transport of all potentials, expressed as net impacts and benefits. Any
materials, products and related energy and water use, as well declared benefits and loads from net flows leaving the product
as waste processing up to the end-of-waste state or disposal of system that have not been allocated as co-products and that
final residues during the use stage. They also include all have passed the end-of-waste state are included in module D.
impacts and aspects related to the losses during the use stage
(i.e. production, transport, and waste processing and disposal Contributions to module D comes from waste incineration
of the lost products and materials). processes in A5 and C3 as well as material recycling in C3. The
specific fractions and net flows are shown in the scenarios
Generally, the geographical coverage of the datasets used section.
matches the actual processes taking place. Meaning, that when
modelling taking place in Grundfos Bjerringbro, the Danish Geographic Representativeness
electricity grid mix is used in the model and thermal energy Land or region, in which the declared product system is
from natural gas. These are generally of very high quality with manufactured, used or handled at the end of the product´s
very good technological, temporal and geographical lifespan: Europe
representativeness.
Comparability
Contributions to operational energy use during the use stage
4 Environmental Product Declaration - Grundfos Holding A/S - MAGNA3 100-80/100/120 (Cast Iron)
Basically, a comparison or an evaluation of EPD data is only into account. Software and databases used: GaBi ts
possible if all the data sets to be compared were created
according to EN 15804 and the building context, respectively 9.2.1.68 (database schema 8007) Ecoinvent v3.5..
the product-specific characteristics of performance, are taken
LCA: Scenarios and additional technical information
An
Characteristic product properties of biogenic carbon estimated RSL of 10 years can be used to facilitate building
The biogenic carbon content quantifies the amount of biogenic calculations. This
carbon in a construction product leaving the factory gate, and it is an EU consensus-based estimation, referenced in Appendix
will be separately declared for the product and for any 7: Lot 11 –
accompanying packaging, as required from the PCR Part A. Circulators in Buildings, prepared by AEA Energy &
The Carbon content of Cardboard and Paper is assumed to Environment for the
0.46 kg C. Overall, there is an amount of 9 weight-% Carbon in European Commission in the context of the Eco Design
the product leaving the factory gate and has to be considered. Directive.
Operational energy use (B6)
Information on describing the biogenic Carbon Content at
Name Value Unit
factory gate
Electricity consumption 2020 kWh/a
Name ValueUnit
Electricity consumption 2790 kWh/a
Biogenic carbon content in accompanying kg
0.74 Electricity consumption 3180 kWh/a
packaging C
Average power input, 0,404 kW
Note: 1 kg of biogenic carbon is equivalent to 44/12 kg of CO2
Average power input, 0,558 kW
Average power input, 0,636 kW
The following technical scenario information is required for the Running hours (all groups) 5.000 h/a
declared modules and optional for non-declared modules.
End of life (C1-C4)
Modules for which no information is declared can be deleted;
additional information can also be listed if necessary. Name Value Unit
Collected as mixed construction waste 34,42 kg
The following technical information is a basis for the declared
Transportation distance (C2) 500 km
modules or can be used for developing specific scenarios in the
Aluminium for recycling 3,43 kg
context of a building assessment if modules are not declared
(MND). Steel for recycling 22,2 kg
Copper for recycling 1,05 kg
A5 is not declared including the disposal of the packaging Stainless steel for recycling 1,04 kg
material on the construction site, the amounts of packaging
Plastics for incineration w/energy 1,58 kg
materials included in the LCA calculations must be declared as
Electronics for incineration w/energy 0,81 kg
technical scenario information for Module A5.
Landfilling 4,31 kg
Reuse, recovery and/or recycling potentials (D), relevant
Transport from the gate to the site (A4) scenario information
Name Value Unit Name ValueUnit
Litres of fuel 0,052 l/100km A5, incineration w/energy recov. (LDPE foil) 6,19 MJ
Transport distance 2003 km A5, incineration w/energy recov. (Paper/Cardboard) 11,2 MJ
Capacity utilisation (including empty runs) 85 % C3, steel for recycling (net amounts) -2,2 kg
Gross density of products transported 716 kg/m3 C3, stainless steel for recycling (net amounts) 0,49 kg
Wastage during distribution 0,02 % C3, aluminium for recycling (net amounts) -0,46 kg
C3, copper for recycling (net amounts) 0,451 kg
Installation into the building (A5)
C3, plastics for incineration, w/ energy recov. 1,58 kg
Name ValueUnit
C3, electronics for incineration, w/ energy recov. 0,81 kg
Packaging waste for incineration (LDPE film) 0,031 kg
Packaging waste for incineration
2,81 kg
(Paper/Cardboard)
5 Environmental Product Declaration - Grundfos Holding A/S - MAGNA3 100-80/100/120 (Cast Iron)
LCA: Results
Characterization model: EN 15804 - 2012+A2 - 2019, PEF. By Decision no. 20170712-n of the IBU SVR, the modules B3, B4, B5 are
marked as MNR (module not relevant) as default. The LCA results in module B6 are given on a period of one year, according to PCR
Part B. To obtain the results from module B6 over the entire life cycle, the LCA results of module B6 must be multiplied by the
estimated RSL of 10 years. The indicator results for module B6 are declared for Group 1. B6 indicator results for other groups can be
derived by multiplying the B6 indicator results with the following factors:
Group 2: 1,38 Group 3: 1,57
DESCRIPTION OF THE SYSTEM BOUNDARY (X = INCLUDED IN LCA; ND = MODULE OR INDICATOR NOT DECLARED; MNR =
MODULE NOT RELEVANT)
Benefits and
Construction loads beyond
Product stage Use stage End of life stage
process stage the system
boundaries
la ire ta m w a Ry lp p u s tro p s n a rT g n iru tc a fu n a M e h t m o rf tro p s n a rTe tis e h t o t e ta g y lb m e s s A e s U e c n a n e tn ia M ria p e R tn e m e c a lp e R tn e m h s ib ru fe R y g re n e la n o ita re p Oe s u re ta w la n o ita re p Oe s u n o itc u rts n o c -e Dn o itilo m e d tro p s n a rT g n is s e c o rp e ts a W la s o p s iD -e s u e R-y re v o c e R-g n ilc y c e Rla itn e to p
A1 A2 A3 A4 A5 B1 B2 B3 B4 B5 B6 B7 C1 C2 C3 C4 D
X X X X X MND MND MNR MNR MNR X MND X X X X X
RESULTS OF THE LCA - ENVIRONMENTAL IMPACT according to EN 15804+A2: 1PCS of MAGNA3 100-80/100/120 (Cast Iron)
Parameter Unit A1 A2 A3 A4 A5 B6 C1 C2 C3 C4 D
GWP-total kg CO 2 eq 1.41E+02 2.13E+00 8.21E-02 2.32E+00 4.06E+00 8.17E+02 0 9.58E-01 8.45E+00 2.17E-01 6.39E-01
GWP-fossil kg CO 2 eq 1.4E+02 2.11E+00 4.84E+00 2.31E+00 1.86E-01 8.13E+02 0 9.52E-01 8.44E+00 2.23E-01 6.45E-01
GWP-
biogenic kg CO 2 eq 8.37E-01 -3.1E-03 -4.8E+00 -4.61E-03 3.88E+00 2.71E+00 0 -1.61E-03 1.04E-02 -6.72E-03 -1.2E-03
GWP-luluc kg CO 2 eq 2.82E-01 1.59E-02 4.23E-02 1.83E-02 1.38E-04 1.18E+00 0 7.74E-03 5.1E-03 1.96E-04 -4.73E-03
kg CFC11
ODP 1.04E-07 3.76E-16 4.08E-09 2.15E-11 7.41E-16 1.79E-11 0 1.76E-16 7.69E-14 5.02E-16 -9.38E-13
eq
AP mol H+ eq 6.48E-01 1.36E-02 1.91E-02 1.34E-02 1.17E-03 1.8E+00 0 5.63E-03 8.53E-03 6.93E-04 -1.8E-02
EP-
kg P eq 1.73E-03 6.03E-06 8.45E-05 7.26E-06 1.7E-07 2.17E-03 0 2.91E-06 1.35E-05 2.43E-05 -5.35E-06
freshwater
EP-marine kg N eq 8.84E-02 5.07E-03 4.09E-03 6.42E-03 4.29E-04 3.99E-01 0 2.71E-03 2.01E-03 1.6E-04 7.86E-05
EP-terrestrial mol N eq 9.3E-01 5.62E-02 4.07E-02 7.1E-02 5.33E-03 4.19E+00 0 3.01E-02 2.21E-02 1.75E-03 1.48E-03
kg NMVOC
POCP 2.77E-01 1.12E-02 1.14E-02 1.22E-02 1.12E-03 1.09E+00 0 5.15E-03 5.49E-03 5.14E-04 -2.66E-05
eq
ADPE kg Sb eq 7.51E-03 1.63E-07 6.1E-05 1.7E-06 1.24E-08 2.35E-04 0 7.74E-08 1.01E-06 1.51E-08 -1.26E-03
ADPF MJ 1.88E+03 2.81E+01 6.68E+01 3.1E+01 1.4E+00 1.43E+04 0 1.28E+01 6.25E+01 3.2E+00 -1.71E+01
m3 world eq
WDP 2.83E+01 1.95E-02 4.57E-01 2.98E-02 5.01E-01 1.77E+02 0 9.33E-03 1.25E+00 -2.46E-03 -8.96E-01
deprived
GWP = Global warming potential; ODP = Depletion potential of the stratospheric ozone layer; AP = Acidification potential of land and water; EP =
Eutrophication potential; POCP = Formation potential of tropospheric ozone photochemical oxidants; ADPE = Abiotic depletion potential for non-fossil
resources; ADPF = Abiotic depletion potential for fossil resources; WDP = Water (user) deprivation potential)
RESULTS OF THE LCA - INDICATORS TO DESCRIBE RESOURCE USE according to EN 15804+A2: 1PCS of MAGNA3 100-
80/100/120 (Cast Iron)
Parameter Unit A1 A2 A3 A4 A5 B6 C1 C2 C3 C4 D
PERE MJ 5.58E+02 1.52E+00 7.07E+01 1.93E+00 2.41E-01 6.34E+03 0 7.38E-01 2.72E+01 2.24E-01 3.34E+00
PERM MJ 0 0 0 0 0 0 0 0 0 0 0
PERT MJ 5.58E+02 1.52E+00 7.07E+01 1.93E+00 2.41E-01 6.34E+03 0 7.38E-01 2.72E+01 2.24E-01 3.34E+00
PENRE MJ 1.88E+03 2.82E+01 6.68E+01 3.11E+01 1.4E+00 1.43E+04 0 1.28E+01 6.25E+01 3.2E+00 -1.69E+01
PENRM MJ 0 0 0 0 0 0 0 0 0 0 0
PENRT MJ 1.88E+03 2.82E+01 6.68E+01 3.11E+01 1.4E+00 1.43E+04 0 1.28E+01 6.25E+01 3.2E+00 -1.69E+01
SM kg 2.94E+01 0 2.38E-01 5.94E-03 0 0 0 0 0 0 0
RSF MJ 1.46E-23 0 0 2.91E-27 0 0 0 0 0 0 0
NRSF MJ 1.71E-22 0 0 3.42E-26 0 0 0 0 0 0 0
FW m3 9.43E-01 1.78E-03 3.65E-02 2.31E-03 1.18E-02 7.33E+00 0 8.6E-04 4.29E-02 4.07E-05 2.55E-02
PERE = Use of renewable primary energy excluding renewable primary energy resources used as raw materials; PERM = Use of renewable primary
energy resources used as raw materials; PERT = Total use of renewable primary energy resources; PENRE = Use of non-renewable primary energy
excluding non-renewable primary energy resources used as raw materials; PENRM = Use of non-renewable primary energy resources used as raw
materials; PENRT = Total use of non-renewable primary energy resources; SM = Use of secondary material; RSF = Use of renewable secondary fuels;
NRSF = Use of non-renewable secondary fuels; FW = Use of net fresh water
RESULTS OF THE LCA – WASTE CATEGORIES AND OUTPUT FLOWS according to EN 15804+A2:
1PCS of MAGNA3 100-80/100/120 (Cast Iron)
6 Environmental Product Declaration - Grundfos Holding A/S - MAGNA3 100-80/100/120 (Cast Iron)
Parameter Unit A1 A2 A3 A4 A5 B6 C1 C2 C3 C4 D
HWD kg 5.79E-04 1.22E-06 1.22E-04 1.54E-06 7.27E-09 5.92E-06 0 5.93E-07 3.01E-08 1.28E-08 -3.09E-04
NHWD kg 5.5E+00 4.37E-03 3.2E-01 6.32E-03 1.32E-01 1.01E+01 0 2.03E-03 8.87E-01 3.66E+00 2.15E+00
RWD kg 8.66E-02 5.06E-05 1.83E-03 8.16E-05 6.75E-05 2.17E+00 0 2.36E-05 9.3E-03 3.83E-05 -2.19E-03
CRU kg 0 0 0 0 0 0 0 0 0 0 0
MFR kg 0 0 0 0 0 0 0 0 2.77E+01 0 0
MER kg 0 0 0 0 0 0 0 0 0 0 0
EEE MJ 0 0 0 0 6.19E+00 0 0 0 8.26E+00 0 0
EET MJ 0 0 0 0 1.12E+01 0 0 0 1.49E+01 0 0
HWD = Hazardous waste disposed; NHWD = Non-hazardous waste disposed; RWD = Radioactive waste disposed; CRU = Components for re-use;
MFR = Materials for recycling; MER = Materials for energy recovery; EEE = Exported electrical energy; EET = Exported thermal energy
RESULTS OF THE LCA – additional impact categories according to EN 15804+A2-optional:
1PCS of MAGNA3 100-80/100/120 (Cast Iron)
Parameter Unit A1 A2 A3 A4 A5 B6 C1 C2 C3 C4 D
Disease
PM 8.37E-06 1.44E-07 2.64E-07 7.95E-08 6.61E-09 1.51E-05 0 3.29E-08 7.19E-08 7.06E-09 -2.92E-07
incidence
IR kBq U235 eq 9.47E+00 7.46E-03 2.89E-01 1.15E-02 1.04E-02 3.56E+02 0 3.48E-03 1.52E+00 5.44E-03 -1.89E-01
ETP-fw CTUe 9.96E+02 2.1E+01 2.06E+01 2.27E+01 7.04E-01 6.12E+03 0 9.55E+00 2.71E+01 2.25E+00 -1.12E+01
HTP-c CTUh 1.64E-06 4.31E-10 6.61E-07 9.35E-10 3.45E-11 1.69E-07 0 1.98E-10 8E-10 1.29E-10 -6.18E-08
HTP-nc CTUh 2.91E-06 2.37E-08 6.59E-08 2.74E-08 1.59E-09 6.22E-06 0 1.13E-08 3.17E-08 1.13E-08 -4.34E-09
SQP SQP 5.7E+02 9.22E+00 1.39E+02 1.07E+01 3.81E-01 4.55E+03 0 4.48E+00 1.97E+01 2.31E-01 -2.66E+01
PM = Potential incidence of disease due to PM emissions; IR = Potential Human exposure efficiency relative to U235; ETP-fw = Potential comparative
Toxic Unit for ecosystems; HTP-c = Potential comparative Toxic Unit for humans (cancerogenic); HTP-nc = Potential comparative Toxic Unit for humans
(not cancerogenic); SQP = Potential soil quality index
Disclaimer 1 – for the indicator 'Potential Human exposure efficiency relative to U235'.
This impact category deals mainly with the eventual impact of low dose ionizing radiation on human health of the nuclear fuel cycle. It
does not consider effects due to possible nuclear accidents, occupational exposure or radioactive waste disposal in underground
facilities. Potential ionizing radiation from the soil, radon and from some construction materials is also not measured by this indicator.
Disclaimer 2 – for the indicators 'abiotic depletion potential for non-fossil resources', 'abiotic depletion potential for fossil resources',
'water (user) deprivation potential, deprivation-weighted water consumption', 'potential comparative toxic unit for ecosystems', 'potential
comparative toxic unit for humans – cancerogenic', 'Potential comparative toxic unit for humans - not cancerogenic', 'potential soil
quality index'. The results of this environmental impact indicator shall be used with care as the uncertainties on these results are high
as there is limited experience with the indicator.
Disclaimer 3: JRC Technical Reports, Version 2, 2018 Page 6, for the indicator "EP-freshwater". This indicator has been calculated as
'kg P eq' as required in the characterization model EUTREND model, Struijs et al., 2009b, as implemented in ReCiPe; This EPD was
created using a software tool.
References
Standards Institut Bauen und Umwelt e.V.: General Instructions for the
EPD programme of Institut Bauen und Umwelt e.V., Version
EN 15804 2.0, Berlin: Institut Bauen und Umwelt e.V., 2021
www.ibu-epd.com
EN 15804:2012+A1 2013, Sustainability of construction works
— Environmental Product Declarations — Core rules for the Standards
product category of construction products.
Machinery Directive
EN 15804 DIRECTIVE 2006/42/EC OF THE EUROPEAN PARLIAMENT
AND OF THE COUNCIL of 17 May
EN 15804:2012+A2:2019+AC:2021, Sustainability of 2006 on machinery
construction works — Environmental Product Declarations —
Core rules for the product category of construction products. Radio Equipment Directive
DIRECTIVE 2014/53/EU OF THE EUROPEAN PARLIAMENT
ISO 14025 AND OF THE COUNCIL of 16 April 2014 on the harmonisation
of the laws of the Member States relating to the making
EN ISO 14025:2011, Environmental labels and declarations — available on the market of radio equipment
Type III environmental declarations — Principles and
procedures. Electromagnetic Compatibility (EMC) Directive
Further References DIRECTIVE 2014/30/EU OF THE EUROPEAN PARLIAMENT
AND OF THE COUNCIL of 26 February 2014 on the
Title of the software/database harmonistion of the laws of the Member States relating to
electromagnetic compatibility
Title of the software/database. Addition to the title, version.
Place: Publisher, Date of publication [Access on access date].
Ecodesign Directive
IBU 2021
DIRECTIVE 2009/125/EC OF THE EUROPEAN PARLIAMENT
7 Environmental Product Declaration - Grundfos Holding A/S - MAGNA3 100-80/100/120 (Cast Iron)
AND OF THE COUNCIL of 21 October 2009 establishing a requirements for stationary circulation pumps for heating and
framework for the setting of ecodesign requirements for energy- service water installations
related products
EN 61000-3-2
EC 641/2009 EN 61000-3-2:2014/2019, Electromagnetic compatibility (EMC)
COMMISSION REGULATION (EC) No 641/2009 of 22 July – Part 3-2: Limits – Limits for harmonic current emissions
2009 implementing Directive 2005/32/EC of the European (equipment input current =16 A per phase)
Parliament and of the Council with regard to ecodesign
requirements for glandless standalone circulators and EN 61000-3-3
glandless circulators integrated in products EN 61000-3-3:2013-08/ A1:2019, Electromagnetic compatibility
(EMC) – Part 3-3:
EC 622/2012 Limits – Limitation of voltage changes, voltage fluctuations and
COMMISSION REGULATION (EU) No 622/2012 of 11 July flicker in public low voltage supply systems, for equipment with
2012 amending Regulation (EC) No 641/2009 with regard to rated current <= 16 A per phase and not subject to conditional
ecodesign requirements for glandless standalone circulators connection
and glandless circulators integrated in products
EN 61000-6-2
DIRECTIVE 2011/65/EU EN 61000-6-2:2008/2019, Electromagnetic compatibility (EMC)
DIRECTIVE 2011/65/EU OF THE EUROPEAN PARLIAMENT – Part 6-2: Generic standards –Immunity for industrial
AND OF THE COUNCIL of 8 June 2011 on the restriction of the environments
use of certain hazardous substances in electrical and electronic
equipment EN 16297-1
EN 16297-1:2012-10, Pumps – Rotodynamic pumps –
DIRECTIVE 2015/863/EU Glandless circulators – Part 1:
DIRECTIVE 2015/863/EU of 31 March 2015 amending General requirements and procedures for testing and
Annex II to Directive 2011/65/EU of the European Parliament calculation of energy efficiency index (EEI)
and of the Council as regards the list of restricted substances
EN 16297-2
ETSI EN 301 489-1 EN 16297-2:2012-10, Pumps – Rotodynamic pumps –
ETSI EN 301 489-1 V2.2.0, Electromagnetic Compatibility Glandless circulators – Part 2: Calculation of energy efficiency
(EMC) standard for radio equipment and services; Part 1: index (EEI) for standalone circulators
Common technical requirements
EN 16297-3
ETSI EN 301 489-17 EN 16297-3:2012, Pumps – Rotodynamic pumps –Glandless
ETSI EN 301 489-17 V3.2.0, Electromagnetic Compatibility circulators – Part 3: Energy efficiency index (EEI) for circulators
(EMC) standard for radio equipment and services; Part 17: integrated in products
Specific conditions for Broadband Data Transmission Systems
ISO 14001
ETSI EN 300 328 V2.1.1 EN ISO 14001:2015-09, Environmental management systems -
ETSI EN 300 328 V2.1.1, Wideband transmission systems; Requirements with guidance for use
Data transmission equipment operating in the 2,4 GHz ISM
band and using wide band modulation techniques ISO 14025
DIN EN /ISO 14025:2011-10, Environmental labels and
EN 809 declarations — Type III environmental declarations —
EN 809:1998-10 + A1:2009, Pumps and pump units for liquids - Principles and procedures
Common safety requirements
EN 15804
EN 55014-1 EN 15804:2012-04+A1 2013, Sustainability of construction
EN 55014-1:2017, Electromagnetic compatibility – works — Environmental Product Declarations — Core rules for
Requirements for household appliances, electric tools and the product category of construction products
similar apparatus – Part 1: Emission
PCR Part A
EN 55014-2 Institut Bauen und Umwelt e.V., Berlin (pub.): Product Category
EN 55014-2:2015, Electromagnetic compatibility – Rules for Building-Related Products and Services, Product
Requirements for household appliances, electric tools Category Rules for Construction Products from the range of
and similar apparatus – Part 2: Immunity – Product family Environmental Product Declarations of Institut Bauen und
standard (CISPR 14-2:2015) Umwelt (IBU), Part A: Calculation Rules for the Life Cycle
Assessment and Requirements on the Project Report, Version
EN 50581:2012 1.7 (2021)
EN 50581:2012, Technical documentation for the assessment
of electrical and electronic products with respect to the PCR Part B
restriction of hazardous substances Institut Bauen und Umwelt e.V., Berlin (pub.): Product Category
Rules for Building-Related Products and Services, Product
EN 60335-1 Category Rules for Construction Products from the range of
EN 60335-1:2012/A11:2014/A13:2017, Household and similar Environmental Product Declarations of Institut Bauen und
electrical appliances – Safety – Part 1:General requirements Umwelt (IBU), Part B: Requirements on the EPD for Pumps for
liquids and liquids with solids, Version 1.0 (2018)
EN 60335-2-51
EN 60335-2-51:2003-03 + A1:2008 + A2:2012, Household and Further references
similar electrical appliances – Safety –Part 2-51: Particular
8 Environmental Product Declaration - Grundfos Holding A/S - MAGNA3 100-80/100/120 (Cast Iron)
CPR Ecoinvent v3.5
REGULATION (EU) No 305/2011 OF THE EUROPEAN
PARLIAMENT AND OF THE COUNCIL of 9 March 2011 laying GaBi ts
down harmonised conditions for the marketing of construction GaBi ts 9.2.1.68 (database schema 8007)
products and repealing Council Directive 89/106/EEC
REACH
CML 2001 Regulation (EC) No 1907/2006 of the European Parliament and
Impact assessment characterization factors Institute of of the Council of 18 December 2006 concerning the
Environmental Sciences, Leiden University, Netherlands Registration, Evaluation, Authorisation and Restriction of
Chemicals (REACH) (Status: 27.06.2018)
ECHA candidate list
Candidate List of substances of very high concern (SVHCs) for SVR
authorisation, European Chemicals Agency (ECHA), Helsinki, Advisory Board (formerly SVA)
Finland Decision no. 20170712-n
Ecoinvent
9 Environmental Product Declaration - Grundfos Holding A/S - MAGNA3 100-80/100/120 (Cast Iron)
Publisher
Institut Bauen und Umwelt e.V. +49 (0)30 3087748- 0
Hegelplatz 1 info@ibu-epd.com
10117 Berlin www.ibu-epd.com
Germany
Programme holder
Institut Bauen und Umwelt e.V. +49 (0)30 3087748- 0
Hegelplatz 1 info@ibu-epd.com
10117 Berlin www.ibu-epd.com
Germany
Author of the Life Cycle Assessment
Grundfos Holding A/S +45 87501400
Poul Due Jensens Vej 7 atomic@grundfos.com
8850 Bjerringbro www.grundfos.com
Denmark
Owner of the Declaration
Grundfos Holding A/S +45 87501400
Poul Due Jensens Vej 7 atomic@grundfos.com
8850 Bjerringbro www.grundfos.com
Denmark
10 Environmental Product Declaration - Grundfos Holding A/S - MAGNA3 100-80/100/120 (Cast Iron)
