ENVIRONMENTAL PRODUCT DECLARATION
as per ISO 14025 and EN 15804+A2
Owner of the Declaration Grundfos Holding A/S
Publisher Institut Bauen und Umwelt e.V. (IBU)
Programme holder Institut Bauen und Umwelt e.V. (IBU)
Declaration number EPD-GRU-20240162-CBA1-EN
Issue date 15/05/2024
Valid to 14/05/2029
MAGNA 3 D 100-40/60 (Cast Iron)
Grundfos Holding A/S
www.ibu-epd.com | https://epd-online.com
General Information
Grundfos Holding A/S MAGNA 3 D 100-40/60 (Cast Iron)
Programme holder Owner of the declaration
IBU – Institut Bauen und Umwelt e.V. Grundfos Holding A/S
Hegelplatz 1 Poul Due Jensens Vej 7
10117 Berlin 8850 Bjerringbro
Germany Denmark
Declaration number Declared product / declared unit
EPD-GRU-20240162-CBA1-EN 1 PCS. of MAGNA 3 D 100-40/60
(D stands for twin-headed)
This declaration is based on the product category rules: Scope:
Pumps for liquids and liquids with solids, 01/08/2021 The declaration applies to 1 piece of MAGNA3 Twin-headed Cast Iron
(PCR checked and approved by the SVR) pump.
The product is produced in Wahlstedt, Germany, and the life cycle
Issue date assessment is based on data collected at the production site. Production
has been modeled using annual production data from 2021-2022. The
15/05/2024
declaration covers two different types of the MAGNA3 100- product
(40/60).
The owner of the declaration shall be liable for the underlying information
Valid to
and evidence; the IBU shall not be liable with respect to manufacturer
14/05/2029 information, life cycle assessment data and evidences.
The EPD was created according to the specifications of EN 15804+A2. In
the following, the standard will be simplified as EN 15804.
Verification
The standard EN 15804 serves as the core PCR
Independent verification of the declaration and data according to ISO
14025:2011
internally X externally
Dipl.-Ing. Hans Peters
(Chairman of Institut Bauen und Umwelt e.V.)
Florian Pronold Mrs Kim Allbury,
(Managing Director Institut Bauen und Umwelt e.V.) (Independent verifier)
1 Environmental Product Declaration - Grundfos Holding A/S - MAGNA 3 D 100-40/60 (Cast Iron)
Product
EN 61000-3-3:2013 A1:2019
Product description/Product definition
The Grundfos MAGNA3 twin-headed circulator pumps are RoHS Directive 2011/65/EU and 2015/863//EU
designed for circulating liquids in heating systems, air
conditioning and cooling systems and domestic hot water Standard: EN 50581:2012.
systems. However, the pump range can also be used in ground
source heat pump systems and solar heating systems. Ecodesign Directive (2009/125/EC)
The MAGNA3 pump is a centrifugal pump powered by an Commission Regulation (EC) No: 641/2009 and
electrical motor. It has a high-performance neodymium magnet
rotor which increases motor efficiency and an insulation shell to Commission Regulation (EU) 622/2012
reduce heat loss from the cast iron pump housing with threaded
connections. Standards used:
EN 16297-1:2012, EN 16297-2:2012, EN 16297-3:2012.
The declaration covers two types of the MAGNA3 pump. They
are grouped as shown below. The group reference in the The CE marking takes into account the proof of conformity with
technical data and scenarios refers also to these. the respective harmonised norms based on the legal provisions
above.
Group 1 MAGNA3 pumps are not harmonised in accordance with the
MAGNA3 D 100-40 F 340 1x230V PN6/10 CPR.
MAGNA3 D 100-40 F 340 1x230V PN16
Group 2 Application
MAGNA3 D 100-60 F 340 1x230V PN6/10 For the application and use the respective national provisions
MAGNA3 D 100-60 F 340 1x230V PN16 apply.
These are all the same physical products and 100 % identical
in terms of design, dimensions and materials as well as supply The pump is designed for circulating liquids in the following
chain and manufacturing processes, i.e., all cradle to gate systems:
processes (A1-A3).
· heating systems
The products are also identical in terms of packaging quality
and materials, distribution, reference service life and end-of-life · domestic hot-water systems
treatment.
· air-conditioning and cooling systems
The only thing that differentiates the products from each other
is the software which controls how the pump operates in the · ground-source heat-pump systems
system in which it is installed, making them fit for different
applications. Hence, all life cycle modules are identical, except · solar-heating systems
use stage module B6, which will change, as the applied
scenarios for electricity consumption changes. The pump is suitable for thin, clean, non-aggressive and non-
explosive liquids, not containing solid particles or fibres that
For the placing on the market in the European Union/European may attack the pump mechanically or chemically. In heating
Free Trade Association (EU/EFTA) (with the exception of systems, the water must meet the requirements of accepted
Switzerland) the following legal provisions apply: standards on water quality. The pumps are also suitable for
domestic hot-water systems.
Machinery Directive (2006/42/EC)
Technical Data
Standard used: EN 809:1998 + A1:2009. The performance data of the product according to the
harmonised norms, based on the harmonisation provisions
Radio Equipment Directive (2014/53/EU) above apply.
The relevant technical specifications according to the PCR Part
Standards used: B are given in the table below.
EN 60335-1:2012/AC:2014 + A11:2014, EN 60335-2-51:2003 + Characteristics that are the same for all three product groups
A1:2008 + A2:2012, EN 62233:2008. are only given once. Others are given individually for all three
groups.
EN 55014-1:2006 + A1:2009 + A2:2011, EN 55014-1:2017, EN Constructional data
61000-6-2:2005, EN 61000-3-2:2014, EN 61000-3-3:2013,
ETSI EN 301 489-1 V2.2.0, ETSI EN 301 489-17 V3.2.0. ETSI
EN 300 328 V2.1.1
Electromagnetic Compatibility (EMC) Directive
(2014/30/EU)
Standards used:
EN 55014-1:2017, EN 55014-2:2015,
EN 61000-3-2:2014/2019, EN 61000-6-2:2008/2019,
2 Environmental Product Declaration - Grundfos Holding A/S - MAGNA 3 D 100-40/60 (Cast Iron)
Name Value Unit REACH
Frequency 50 Hz
This product/article/at least one partial article contains
Voltage 230 V
substances listed in the ECHA candidate list (date:10.06.2022)
Clean
Pumped liquid (e.g. water) - exceeding 0.1 percentage by mass: no
Water
The Wahlstedt production has been assessed and certified as
Energy Efficiency Index Gr.1 0,17 meeting the requirements in ISO 14001, ISO 50001, ISO 45001
Energy Efficiency Index Gr. 2 0,17 and ISO 9001.
Flow range Gr. 1 (max) 50 m3/h
Reference service life
Flow range Gr. 2 (max) 53 m3/h No use stage scenario which refers to the lifetime of the product
Head max. Gr.1 4 m is declared. However, to facilitate building calculations, an
Head max. Gr.2 6 m estimated RSL of 10 years can be used.
This is an EU consensus-based estimation, referenced on page
Power input Gr. 1 Average (from load profile
0,204 kW 37 in Appendix 7: Lot 11 – Circulators in Buildings, prepared by
describing use)
AEA Energy & Environment for the European Commission in
Power input Gr. 2 Average (from load profile
0,257 kW the context of the Eco Design Directive:
describing use)
Nominal capacity Gr.1 0,452 kW There is no definitive information on the average circulator life
Nominal capacity Gr. 2 0,65 kW available, there is consensus within the industry that it is at
least 12 years. However, this is complicated by many factors,
Performance data of the product according to the harmonised
including many being scrapped prematurely when e.g. the
standards, based on provisions for harmonisation.
boiler they are connected to is replaced.
Base materials/Ancillary materials
From the estimated stock (140Mpa) and annual sales (14Mpa),
Base materials / Ancillary materials
the average lifetime of the circulator is taken as 10 years for the
Name Value Unit purposes of this study.
Aluminium 9,77 %
Cast iron 59,45 % The RSL of the declared product is not directly influencing the
results in this study, as no declared use stage scenario is
Carbon steel 9,05 %
dependent on the RSL; The use stage sub-module B6 is
Ceramics 0,21 %
declared per year as required by the PCR Part B.
Copper 3,66 %
Electronics (including PCB) 2,82 %
Magnet Nd 0,77 %
Paper 0,18 %
Plastics 0,26 %
Plastics, foam 0,73 %
Plastics GF 3,74 %
Rubber 0,46 %
Stainless steel 3,9 %
Cardboard 4,93 %
Plastic film 0,04 %
TOTAL 100 %
LCA: Calculation rules
of the EPD follow the modular approach in EN 15804. By
Declared Unit decision no. 20170712-n of the SVR, the modules B3, B4 and
The declared unit is 1 piece (pcs.) of MAGNA3 D Cast Iron B5 are by default declared as "MNR" (module not relevant).
pump and it also includes the packaging.
Declared unit The product stage (A1-A3) comprises raw material extraction
and processing, transport processes as well as the
Name Value Unit
manufacturing process. The final production and assembly of
Declared unit 1 pce.
the MAGNA3 pump takes place at a Grundfos manufacturing
Mass reference 64.602 kg/pce site in Germany. However, the full supply-chain leading to the
Conversion factor [Mass/Declared Unit] 64.602 - finished product at the gate is rather complex and includes a
large amount of raw materials, components and semi-finished
Other declared units are allowed if the conversion is shown
parts which come from both external suppliers as well as other
transparently.
Grundfos production facilities
System boundary The product stage is included in the study, and according to EN
15804 the system boundary with nature is set to include those
System boundary
processes that provide the material and energy inputs into the
system and the following manufacturing, transport up to the
factory gate as well as the processing of any waste arising from
This EPD is Cradle-To-Grave. The system boundaries
those processes.
3 Environmental Product Declaration - Grundfos Holding A/S - MAGNA 3 D 100-40/60 (Cast Iron)
Wastes and losses are included in the modules where they
occur according to the polluter pays principle and the modular · Transport of packaging waste to the treatment site;
approach of EN 15804.
· Waste treatment of packaging.
The product includes:
The packaging material does not reach the end of waste state
· A1 Extraction and processing of raw materials; but is incinerated as waste. According to European statistics,
the average R1 value of incineration plants is > 0.6. Therefore,
· A1 Reuse of products or materials from a previous product it is assumed that packaging material is treated thermally in an
system; incineration plant with R1 > 0.6. The loads from the combustion
process of packaging are declared in module A5 and the
· A1 Processing of secondary materials; resulting energy benefits in module D, as required by the PCR
Part A, 5.5.2.
· A1 Generation of electricity, steam and heat from primary
energy resources, also including their extraction, refining and Use stage (B1-B7):
transport;
The use stage, related to the building fabric includes:
· A1 Energy recovery and other recovery processes from
secondary fuels; · B1, use or application of the installed product;
· A2 Transportation up to the factory gate and internal transport; · B2, maintenance.
· A3 Production of ancillary materials or pre products; The use stage related to the operation of the building includes:
· A3 Manufacturing of products and coproducts; · B6, operational energy use;
· A3 Manufacturing of packaging; · B7, operational water use.
· A1-A3 processing up to the end-of-waste state or disposal of In this study, all use stage modules are assessed, though B1,
final residues. B2 and B7 are assessed to be zero. By decision no. 20170712-
n of the SVR, the modules B3, B4 and B5 are by default
For secondary material inputs, the system boundary to the declared as "MNR" (module not relevant).
previous system (providing the secondary material) is set where The modules include the provision and transport of all
outputs reach the end-of-waste state. The recycling of materials, products and related energy and water use, as well
secondary material into new raw materials is included in the as waste processing up to the end-of-waste state or disposal of
system boundary of this study. Waste final residues during the use stage. They also include all
impacts and aspects related to the losses during the use stage
materials from production processes that are recycled without (i.e. production, transport, waste processing and disposal of the
any modification of the material's inherent characteristics are lost products and materials).
modelled as closed-loop within A1-A3. This is done up to the
input mass flow that was used during production. Generally, the geographical coverage of the datasets used
matches the actual processes taking place. Meaning, that when
Waste for incineration arising in the product stage is accounted modelling taking place in Grundfos Bjerringbro, the Danish
for in the module where the waste is produced. The electricity grid mix is used in the model and thermal energy
environmental loads from the incineration process are declared from natural gas. These are generally of very high quality with
in the module where it occurs and the electricity and heat which very good technological, temporal and geographical
is produced from the incineration are considered as closed-loop representativeness.
within A1-A3, as described in PCR Part A, 5.5.1. The input of
biogenic carbon from the production of packaging material is Contributions to operational energy use during the use stage
inventoried in A3. As required by PCR Part A, the (B6) come from the electricity consumption of the product. The
corresponding end-of-life module of the packaging material, A5, annual electricity consumption is calculated by multiplying the
is also declared and the emissions of biogenic carbon are average power input, which is based on a defined load profile,
inventoried. with the annual running hours. For use stage (B6) European
Average electricity grid mix has been used. These values are
The construction process stage (A4-A5) includes: declared in the scenarios section.
A4: The End-of-Life stage (C1-C4) includes all activities from
when the product reaches the end of its service life and no
· Transportation from factory gate to the distribution centre: longer provides any functionality and until all materials and
components are processed for reuse/recycling or disposed of.
· Consumption of electricity, thermal energy and water at the
distribution centre; According to EN 15804 and the PCR Part A, the end-of-life
stage includes:
· Transportation from distribution centre to construction site;
· C1 deconstruction of the product from the building, including
· Wastage during distribution. initial on-site sorting of the materials;
A5: · C2 transportation of the discarded product to a recycling site
and transportation of waste to final disposal;
· Installation process;
4 Environmental Product Declaration - Grundfos Holding A/S - MAGNA 3 D 100-40/60 (Cast Iron)
· C3 waste processing, collection of waste fractions from the potentials, expressed as net impacts and benefits. Any
deconstruction and waste processing of material flows intended declared benefits and loads from net flows leaving the product
for reuse, recycling and energy recovery; system that have not been allocated as co-products and that
have passed the end-of waste state are included in module D.
· C4 waste disposal including physical pretreatment and
management of the disposal site. Contributions to module D comes from waste incineration
processes in A5 and C3 as well as material recycling in C3. The
At end of life, the MAGNA3 pump is manually disassembled specific fractions and net flows are shown in the scenarios
from the piping system in which it has been installed. The section.
definition of the applied end-of-life scenario in this EPD follows
the requirements in the Comparability
PCR Part A, 6.2 regarding complex products, with a Basically, a comparison or an evaluation of EPD data is only
combination of recycling, thermal waste treatment and possible if all the data sets to be compared were created
landfilling. 100 % of the material is considered in the end of life according to EN 15804 and the building context, respectively
scenario as required by the PCR. An overall collection rate of the product-specific characteristics of performance, are taken
90 % has been assumed. into account.
Materials from which energy is recovered in an incineration
process with an R1-value above 0.60 are in this study included Geographic Representativeness
with the environmental burdens from the incineration process Land or region, in which the declared product system is
inventoried in C3, the recovered energy is declared as exported manufactured, used or handled at the end of the product´s
energy in C3 and the energy benefits are declared in D. This lifespan: Germany
procedure is according to the PCR Part A, 5.5.6. C3 includes
the mechanical separation of the product followed by a series
Comparability
of sorting steps. Metal fractions are recycled and plastics,
Basically, a comparison or an evaluation of EPD data is only
cardboard and electronics are assumed incinerated with energy
possible if all the data sets to be compared were created
recovery. The residual fractions are landfilled and declared in
according to EN 15804 and the building context, respectively
C4.
the product-specific characteristics of performance, are taken
into account. Software and databases used: LCA for Experts
The specific amounts are shown in the scenarios section.
10.7.1.28
Schema 8007
Beyond system boundary (D): According to EN 15804
Sphera and Ecoinvent databases
module D includes the reuse, recovery and/or recycling
LCA: Scenarios and additional technical information
Name ValueUnit
Characteristic product properties of biogenic carbon
Packaging waste for incineration (LDPE film) 0,028 kg
The biogenic carbon content quantifies the amount of biogenic
Packaging waste for incineration
carbon in a construction product leaving the factory gate, and it 3,301 kg
(Paper/Cardboard)
will be separately declared for the product and for any
accompanying packaging, as required from the PCR Part A. An estimated RSL of 10 years can be used to facilitate building
The carbon content of cardboard and paper is assumed to calculations. This is an EU consensus-based estimation,
46%. Overall, there is an amount of weight-% Carbon in the referenced in Appendix 7: Lot 11 – Circulators in Buildings,
product leaving the factory gate and has to be considered prepared by AEA Energy & Environment for the European
Information on describing the biogenic Carbon Content at Commission in the context of the Eco Design Directive.
factory gate Reference service life
Note: 1 kg of biogenic carbon is equivalent to 44/12 kg of CO2. Name Value Unit
Name ValueUnit Life Span according to the manufacturer 10 a
kg
Biogenic carbon content in product - C Operational energy use (B6)
Biogenic carbon content in accompanying kg Name Value Unit
1.52
packaging C Electricity consumption Group 1 1020 kWh/a
Electricity consumption Group 2 1285 kWh/a
Average power input, Group 1 0,204 kW
Transport from the gate to the site (A4) Average power input, Group 2 0,257 kW
Name Value Unit Running hours (all groups) 5.000 h/a
Litres of fuel 0,0524 l/100km
End of life (C1-C4)
Transport distance 2003 km
Capacity utilisation (including empty runs) 85 %
Gross density of products transported 704 kg/m3
Wastage during distribution 0,02 %
Installation into the building (A5)
5 Environmental Product Declaration - Grundfos Holding A/S - MAGNA 3 D 100-40/60 (Cast Iron)
Name Value Unit Reuse, recovery and/or recycling potentials (D), relevant
Collected as mixed construction waste 61,273 kg scenario information
Transportation distance (C2) 500 km Name Value Unit
Aluminium for recycling 5,57 kg A5, incineration w/energy recov. thermal energy 13,1 MJ
Steel for recycling 39,03 kg A5, incineration w/energy recov. electric energy 7,21 MJ
Copper for recycling 2,09 kg C3, steel for recycling (net amounts) -3,34 kg
Stainless steel for recycling 2,22 kg C3, stainless steel for recycling (net amounts) 1,01 kg
Plastics for incineration w/energy 2,96 kg C3, aluminium for recycling (net amounts) -0,88 kg
Electronics for incineration w/energy 1,61 kg C3, copper for recycling (net amounts) 0,892 kg
Landfilling 7,79 kg C3, incineration w/energy recov. thermal energy 28,2 MJ
C3, incineration w/energy recov. electric energy. 15,6 MJ
6 Environmental Product Declaration - Grundfos Holding A/S - MAGNA 3 D 100-40/60 (Cast Iron)
LCA: Results
Characterization model: EN 15804 - 2012+A2 - 2019, PEF. By Decision no. 20170712-n of the IBU SVR, the modules B3, B4, B5 are
marked as MNR (module not relevant) as default. The LCA results in module B6 are given over a period of one year, according to PCR
Part B. To obtain the results from module B6 over the entire life cycle, the LCA results of module B6 must be multiplied by the
estimated RSL of 10 years. The indicator results for module B6 are declared for Group 1. B6 indicator results for other groups can be
derived by multiplying the B6 indicator results with the following factors:
Group 2: 1,259
DESCRIPTION OF THE SYSTEM BOUNDARY (X = INCLUDED IN LCA; MND = MODULE OR INDICATOR NOT DECLARED; MNR
= MODULE NOT RELEVANT)
Benefits and
Construction loads beyond
Product stage Use stage End of life stage
process stage the system
boundaries
la ire ta m w a Ry lp p u s tro p s n a rT g n iru tc a fu n a M e h t m o rf tro p s n a rTe tis e h t o t e ta g y lb m e s s A e s U e c n a n e tn ia M ria p e R tn e m e c a lp e R tn e m h s ib ru fe R y g re n e la n o ita re p Oe s u re ta w la n o ita re p Oe s u n o itc u rts n o c -e Dn o itilo m e d tro p s n a rT g n is s e c o rp e ts a W la s o p s iD -e s u e R-y re v o c e R-g n ilc y c e Rla itn e to p
A1 A2 A3 A4 A5 B1 B2 B3 B4 B5 B6 B7 C1 C2 C3 C4 D
X X X X X X X MNR MNR MNR X X X X X X X
RESULTS OF THE LCA - ENVIRONMENTAL IMPACT according to EN 15804+A2: 1PCS of MAGNA 3 D 100-40/60
Parameter Unit A1 A2 A3 A4 A5 B1 B2 B6 B7 C1 C2 C3 C4 D
GWP-total kg CO 2 eq 2.25E+02 4.64E+00 1.84E+00 4.93E+00 4.75E+00 0 0 3.32E+02 0 0 2.1E+00 1.44E+01 3.81E-01 1.43E+00
GWP-fossil kg CO 2 eq 2.23E+02 4.66E+00 7.4E+00 4.95E+00 1.9E-01 0 0 3.29E+02 0 0 2.12E+00 1.43E+01 3.86E-01 1.44E+00
GWP- -5.62E
biogenic kg CO 2 eq 1.92E+00 -6.23E-02 +00 -7.23E-02 4.56E+00 0 0 2.86E+00 0 0 -3.13E-02 4.25E-02 -4.76E-03 -7.56E-03
GWP-luluc kg CO 2 eq 2.8E-01 3.94E-02 5.89E-02 4.51E-02 1.43E-04 0 0 3.58E-02 0 0 1.96E-02 6.2E-04 3.48E-04 -7.02E-03
kg CFC11
ODP 1.28E-07 5.81E-13 8.11E-09 2.82E-11 5.88E-13 0 0 6.07E-09 0 0 2.76E-13 9.22E-11 6.45E-13 -6.16E-11
eq
AP mol H+ eq 1.17E+00 3.14E-02 3.55E-02 2.95E-02 1.37E-03 0 0 7.03E-01 0 0 1.27E-02 1.23E-02 1.19E-03 -4.23E-02
EP-
kg P eq 3.31E-03 1.56E-05 1.2E-04 1.85E-05 2.29E-07 0 0 1.23E-03 0 0 7.75E-06 2.61E-05 4.44E-05 -1.29E-05
freshwater
EP-marine kg N eq 1.55E-01 1.14E-02 7.4E-03 1.43E-02 5.09E-04 0 0 1.68E-01 0 0 6.2E-03 3.12E-03 2.84E-04 -4.68E-04
EP-terrestrial mol N eq 1.62E+00 1.26E-01 7.45E-02 1.58E-01 6.31E-03 0 0 1.76E+00 0 0 6.88E-02 3.46E-02 3.12E-03 -3.19E-03
kg
POCP NMVOC 4.72E-01 2.52E-02 2.09E-02 2.72E-02 1.32E-03 0 0 4.49E-01 0 0 1.18E-02 8.35E-03 8.97E-04 -2.1E-03
eq
ADPE kg Sb eq 1.83E-02 2.86E-07 1.14E-04 4E-06 6.17E-09 0 0 5.09E-05 0 0 1.41E-07 7.71E-07 1.04E-08 -2.6E-03
ADPF MJ 3.22E+03 6.29E+01 1.1E+02 6.78E+01 1.68E+00 0 0 6.92E+03 0 0 2.89E+01 1.07E+02 5.77E+00 -2.14E+01
m3 world
WDP eq 5.93E+01 5.21E-02 3.32E-01 7.43E-02 5.86E-01 0 0 7.33E+01 0 0 2.56E-02 2.05E+00 -5.37E-03 -1.32E+00
deprived
GWP = Global warming potential; ODP = Depletion potential of the stratospheric ozone layer; AP = Acidification potential of land and water; EP =
Eutrophication potential; POCP = Formation potential of tropospheric ozone photochemical oxidants; ADPE = Abiotic depletion potential for non-fossil
resources; ADPF = Abiotic depletion potential for fossil resources; WDP = Water (user) deprivation potential)
RESULTS OF THE LCA - INDICATORS TO DESCRIBE RESOURCE USE according to EN 15804+A2: 1PCS of MAGNA 3 D 100-
40/60
Parameter Unit A1 A2 A3 A4 A5 B1 B2 B6 B7 C1 C2 C3 C4 D
PERE MJ 1.38E+03 4.24E+00 1E+02 5.32E+00 3.76E-01 0 0 4.14E+03 0 0 2.1E+00 6.28E+01 5.2E-01 -3.01E-01
PERM MJ 0 0 0 0 0 0 0 0 0 0 0 0 0 0
PERT MJ 1.38E+03 4.24E+00 1E+02 5.32E+00 3.76E-01 0 0 4.14E+03 0 0 2.1E+00 6.28E+01 5.2E-01 -3.01E-01
PENRE MJ 3.23E+03 6.31E+01 1.1E+02 6.8E+01 1.68E+00 0 0 6.93E+03 0 0 2.9E+01 1.07E+02 5.78E+00 -2.08E+01
PENRM MJ 0 0 0 0 0 0 0 0 0 0 0 0 0 0
PENRT MJ 3.23E+03 6.31E+01 1.1E+02 6.8E+01 1.68E+00 0 0 6.93E+03 0 0 2.9E+01 1.07E+02 5.78E+00 -2.08E+01
SM kg 5.12E+01 0 4.76E-01 1.03E-02 0 0 0 0 0 0 0 0 0 0
RSF MJ 2.91E-23 0 0 5.83E-27 0 0 0 0 0 0 0 0 0 0
NRSF MJ 3.42E-22 0 0 6.85E-26 0 0 0 0 0 0 0 0 0 0
FW m3 1.93E+00 4.65E-03 4.75E-02 5.81E-03 1.38E-02 0 0 3.34E+00 0 0 2.3E-03 7.25E-02 6.02E-05 5.23E-02
PERE = Use of renewable primary energy excluding renewable primary energy resources used as raw materials; PERM = Use of renewable primary
energy resources used as raw materials; PERT = Total use of renewable primary energy resources; PENRE = Use of non-renewable primary energy
excluding non-renewable primary energy resources used as raw materials; PENRM = Use of non-renewable primary energy resources used as raw
materials; PENRT = Total use of non-renewable primary energy resources; SM = Use of secondary material; RSF = Use of renewable secondary fuels;
NRSF = Use of non-renewable secondary fuels; FW = Use of net fresh water
7 Environmental Product Declaration - Grundfos Holding A/S - MAGNA 3 D 100-40/60 (Cast Iron)
RESULTS OF THE LCA – WASTE CATEGORIES AND OUTPUT FLOWS according to EN 15804+A2:
1PCS of MAGNA 3 D 100-40/60
Parameter Unit A1 A2 A3 A4 A5 B1 B2 B6 B7 C1 C2 C3 C4 D
HWD kg 9.95E-04 1.96E-10 2.42E-04 2.48E-07 4.74E-11 0 0 -5.42E-07 0 0 8.98E-11 -8.01E-09 4.82E-10 -6.3E-04
NHWD kg 1.16E+01 9.32E-03 7.22E-01 1.32E-02 1.53E-01 0 0 5.07E+00 0 0 4.42E-03 1.62E+00 6.68E+00 4.15E+00
RWD kg 1.57E-01 1.15E-04 3.4E-03 1.71E-04 7.97E-05 0 0 1.1E+00 0 0 5.43E-05 1.67E-02 6.79E-05 -2.73E-03
CRU kg ND ND ND ND ND ND ND ND ND ND ND ND ND ND
MFR kg 0 0 0 0 0 0 0 0 0 0 0 4.89E+01 0 0
MER kg ND ND ND ND ND ND ND ND ND ND ND ND ND ND
EEE MJ 0 0 0 0 7.21E+00 0 0 0 0 0 0 1.56E+01 0 0
EET MJ 0 0 0 0 1.31E+01 0 0 0 0 0 0 2.82E+01 0 0
HWD = Hazardous waste disposed; NHWD = Non-hazardous waste disposed; RWD = Radioactive waste disposed; CRU = Components for re-use;
MFR = Materials for recycling; MER = Materials for energy recovery; EEE = Exported electrical energy; EET = Exported thermal energy
RESULTS OF THE LCA – additional impact categories according to EN 15804+A2-optional:
1PCS of MAGNA 3 D 100-40/60
Parameter Unit A1 A2 A3 A4 A5 B1 B2 B6 B7 C1 C2 C3 C4 D
Disease
PM 1.53E-05 3.73E-07 5.38E-07 1.89E-07 7.63E-09 0 0 5.92E-06 0 0 8.07E-08 1.04E-07 1.21E-08 -6.42E-07
incidence
kBq U235
IR 1.89E+01 1.71E-02 5.45E-01 2.48E-02 1.26E-02 0 0 1.83E+02 0 0 8.09E-03 2.77E+00 1E-02 -1.65E-01
eq
ETP-fw CTUe 1.47E+03 4.5E+01 3.81E+01 4.78E+01 7.58E-01 0 0 1.92E+03 0 0 2.07E+01 3.06E+01 3.63E+00 -1.04E+01
HTP-c CTUh 3.39E-06 9.07E-10 1.32E-06 1.92E-09 4.21E-11 0 0 1.02E-07 0 0 4.21E-10 1.69E-09 2.33E-10 -1.29E-07
HTP-nc CTUh 3.08E-06 3.95E-08 7.92E-08 4.37E-08 1.15E-09 0 0 1.62E-06 0 0 1.87E-08 3.28E-08 1.99E-08 -2.59E-08
SQP SQP 1.17E+03 2.42E+01 1.87E+02 2.81E+01 5.07E-01 0 0 2.72E+03 0 0 1.21E+01 4.15E+01 5.16E-01 -5.39E+01
PM = Potential incidence of disease due to PM emissions; IR = Potential Human exposure efficiency relative to U235; ETP-fw = Potential comparative
Toxic Unit for ecosystems; HTP-c = Potential comparative Toxic Unit for humans (cancerogenic); HTP-nc = Potential comparative Toxic Unit for humans
(not cancerogenic); SQP = Potential soil quality index
Disclaimer 1 – for the indicator 'Potential Human exposure efficiency relative to U235'. This impact category deals mainly with the
eventual impact of low-dose ionizing radiation on human health of the nuclear fuel cycle. It does not consider effects due to possible
nuclear accidents, occupational exposure or radioactive waste disposal in underground facilities. Potential ionizing radiation from the
soil, from radon and from some construction materials is also not measured by this indicator. Disclaimer 2 – for the indicators 'abiotic
depletion potential for non-fossil resources', 'abiotic depletion potential for fossil resources', 'water (user) deprivation potential,
deprivation-weighted water consumption', 'potential comparative toxic unit for ecosystems', 'potential comparative toxic unit for humans
– cancerogenic', 'Potential comparative toxic unit for humans - not cancerogenic', 'potential soil quality index'. The results of this
environmental impact indicator shall be used with care as the uncertainties on these results are high as there is limited experience with
the indicator.
Disclaimer 3: JRC Technical Reports, Version 2, 2018 Page 6, for the indicator "EP-freshwater". This indicator has been calculated as
'kg P eq' as required in the characterization model EUTREND model, Struijs et al., 2009b, as implemented in ReCiPe; This EPD was
created using a software tool.
References
Standards
States relating to electromagnetic compatibility
Machinery Directive
Ecodesign Directive
DIRECTIVE 2006/42/EC OF THE EUROPEAN
DIRECTIVE 2009/125/EC OF THE EUROPEAN
PARLIAMENT AND OF THE COUNCIL of 17 May
PARLIAMENT AND OF THE COUNCIL of 21 October
2006 on machinery
2009 establishing a framework for the setting of
Radio Equipment Directive
ecodesign requirements for energy-related products
DIRECTIVE 2014/53/EU OF THE EUROPEAN PARLIAMENT
AND OF THE COUNCIL of 16 April 2014 on the harmonization EC 641/2009
of the laws of the Member States relating to the making
available on the market of COMMISSION REGULATION (EC) No 641/2009 of 22 July
2009 implementing Directive 2005/32/EC of the European
radio equipment Parliament and of the Council with regard to ecodesign
requirements for glandless standalone circulators and
Electromagnetic Compatibility (EMC) Directive glandless circulators integrated in
DIRECTIVE 2014/30/EU OF THE EUROPEAN products
PARLIAMENT AND OF THE COUNCIL of 26 February EC 622/2012
2014 on the harmonization of the laws of the Member COMMISSION REGULATION (EU) No 622/2012 of 11 July
8 Environmental Product Declaration - Grundfos Holding A/S - MAGNA 3 D 100-40/60 (Cast Iron)
2012 amending Regulation (EC) No 641/2009 with regard to respect to the restriction of hazardous substances
ecodesign requirements for glandless standalone circulators
and glandless circulators integrated in products EN 60335-1
DIRECTIVE 2011/65/EU EN 60335-1:2012/A11:2014/A13:2017, Household
DIRECTIVE 2011/65/EU OF THE EUROPEAN and similar electrical appliances – Safety – Part 1:General
requirements
PARLIAMENT AND OF THE COUNCIL of 8 June 2011
EN 60335-2-51
on the restriction of the use of certain hazardous
EN 60335-2-51:2003-03 + A1:2008 + A2:2012, Household and
substances in electrical and electronic equipment similar electrical appliances – Safety –Part 2-51: Particular
requirements for stationary circulation pumps for heating and
DIRECTIVE 2015/863/EU service water installations
DIRECTIVE 2015/863/EU of 31 March 2015 amending EN 61000-3-2
Annex II to Directive 2011/65/EU of the European EN 61000-3-2:2014/2019, Electromagnetic compatibility (EMC)
– Part 3-2: Limits – Limits for harmonic current emissions
Parliament and of the Council as regards the list of (equipment input current =16 A per phase)
restricted substances EN 61000-3-3
ETSI EN 301 489-1 EN 61000-3-3:2013-08/ A1:2019, Electromagnetic compatibility
(EMC) – Part 3-3:
ETSI EN 301 489-1 V2.2.0, Electromagnetic Compatibility Limits – Limitation of voltage changes, voltage fluctuations and
(EMC) standard for radio equipment and services; Part 1: flicker in public low voltage supply systems, for equipment with
Common technical requirements
rated current <= 16 A per phase and not subject to conditional
ETSI EN 301 489-17 connection
ETSI EN 301 489-17 V3.2.0, Electromagnetic Compatibility EN 61000-6-2
(EMC) standard for radio equipment and services; Part 17:
Specific conditions for Broadband Data Transmission Systems EN 61000-6-2:2008/2019, Electromagnetic compatibility (EMC)
– Part 6-2: Generic standards –Immunity for industrial
ETSI EN 300 328 V2.1.1 environments
ETSI EN 300 328 V2.1.1, Wideband transmission systems; EN 16297-1
Data transmission equipment operating in the 2,4 GHz ISM
band and using wide band modulation techniques EN 16297-1:2012-10, Pumps – Rotodynamic pumps –
Glandless circulators – Part 1:
EN 809 General requirements and procedures for testing and
calculation of energy efficiency index (EEI)
EN 809:1998-10 + A1:2009, Pumps and pump units for
EN 16297-2
liquids - Common safety requirements
EN 16297-2:2012-10, Pumps – Rotodynamic pumps –
EN 55014-1 Glandless circulators – Part 2: Calculation of energy efficiency
index (EEI) for standalone circulators
EN 55014-1:2017, Electromagnetic compatibility –
Requirements for household appliances, electric tools and EN 16297-3
similar apparatus – Part 1: Emission
EN 16297-3:2012, Pumps – Rotodynamic pumps –Glandless
EN 55014-2 circulators – Part 3: Energy efficiency index (EEI) for circulators
integrated in products
EN 55014-2:2015, Electromagnetic compatibility –
ISO 14001
Requirements for household appliances, electric tools
EN ISO 14001:2015-09, Environmental management systems -
and similar apparatus – Part 2: Immunity – Product Requirements with guidance for use
family standard (CISPR 14-2:2015) ISO 14025
EN 50581:2012 DIN EN /ISO 14025:2011-10, Environmental labels and
declarations — Type III environmental declarations —
EN 50581:2012, Technical documentation for the Principles and procedures
assessment of electrical and electronic products with EN 15804
9 Environmental Product Declaration - Grundfos Holding A/S - MAGNA 3 D 100-40/60 (Cast Iron)
EN 15804:2012-04+A1 2013, Sustainability of construction Finland
works — Environmental Product Declarations — Core rules for
the product category of construction products EUTREND model
PCR Part A Struijs et al., 2009b
AEA Energy & Environment
Institut Bauen und Umwelt e.V., Berlin (pub.): Product Category
Rules for Building-Related Products and Services, Product Circulators in Buildings
Category Rules for Construction Products from the range of
Environmental Product Declarations of Institut Bauen und Ecoinvent
Umwelt (IBU), Part A: Calculation Rules for the Life Cycle
Assessment and Requirements on the Project Report, Version
1.3. Ecoinvent v3.9.1
PCR Part B LCA for Experts
Institut Bauen und Umwelt e.V., Berlin (pub.): Product Category LCA for Experts 10.7.1.28Schema 8007
Rules for Building-Related Products and Services, Product
Category Rules for Construction Products from the range of REACH
Environmental Product Declarations of Institut Bauen und
Umwelt (IBU), Part B: Requirements on the EPD for Pumps for Regulation (EC) No 1907/2006 of the European Parliament and
liquids and liquids with solids, Version 1.0 (2018) of the Council of 18 December 2006 concerning the
Registration, Evaluation, Authorisation and Restriction of
Further references Chemicals (REACH) (Status: 27.06.2018)
CPR SVR
REGULATION (EU) No 305/2011 OF THE EUROPEAN Advisory Board (formerly SVA)
PARLIAMENT AND OF THE COUNCIL of 9 March 2011 laying
down harmonised conditions for the marketing of construction Decision no.
products and repealing Council Directive 89/106/EEC 20170712-n
CML 2001 AEA Energy & Environment
ED02287 Circulators in buildings for the European Commission
Impact assessment characterization factors Institute of
Environmental Sciences, Leiden University, Netherlands EUTREND model, Struijs et al., 2009b[BSJ1] ,
ECHA candidate list EUTREND model
Struijs et al 2009b
Candidate List of substances of very high concern (SVHCs) for
authorisation, European Chemicals Agency (ECHA), Helsinki,
10 Environmental Product Declaration - Grundfos Holding A/S - MAGNA 3 D 100-40/60 (Cast Iron)
Publisher
Institut Bauen und Umwelt e.V. +49 (0)30 3087748- 0
Hegelplatz 1 info@ibu-epd.com
10117 Berlin www.ibu-epd.com
Germany
Programme holder
Institut Bauen und Umwelt e.V. +49 (0)30 3087748- 0
Hegelplatz 1 info@ibu-epd.com
10117 Berlin www.ibu-epd.com
Germany
Author of the Life Cycle Assessment
Grundfos Holding A/S +45 87501400
Poul Due Jensens Vej 7 LCA_EPD@grundfos.com
8850 Bjerringbro www.grundfos.com
Denmark
Owner of the Declaration
Grundfos Holding A/S +45 87501400
Poul Due Jensens Vej 7 LCA_EPD@grundfos.com
8850 Bjerringbro www.grundfos.com
Denmark
11 Environmental Product Declaration - Grundfos Holding A/S - MAGNA 3 D 100-40/60 (Cast Iron)
