ENVIRONMENTAL PRODUCT DECLARATION
as per ISO 14025 and EN 15804+A2
Owner of the Declaration Grundfos Holding A/S
Publisher Institut Bauen und Umwelt e.V. (IBU)
Programme holder Institut Bauen und Umwelt e.V. (IBU)
Declaration number EPD-GRU-20230052-CBC2-EN
Issue date 31.08.2023
Valid to 30.08.2028
MAGNA3 50-40/60/80 (Cast Iron)
Grundfos Holding A/S
www.ibu-epd.com | https://epd-online.com
General Information
Grundfos Holding A/S MAGNA3 50-40/60/80 (Cast Iron)
Programme holder Owner of the declaration
IBU – Institut Bauen und Umwelt e.V. Grundfos Holding A/S
Hegelplatz 1 Poul Due Jensens Vej 7
10117 Berlin 8850 Bjerringbro
Germany Denmark
Declaration number Declared product / declared unit
EPD-GRU-20230052-CBC2-EN 1 PCS. of MAGNA3 50-40/60/80 (Cast Iron)
This declaration is based on the product category rules: Scope:
Pumps for liquids and liquids with solids, 01.08.2021 The declaration applies to 1 piece of MAGNA3 (Cast Iron) pump.
(PCR checked and approved by the SVR)
The product is produced in Wahlstedt, Germany, and the life cycle
assessment is based on data collected at the production site. Production
Issue date has been modeled using annual production data from 2021. The
declaration covers three different types of the MAGNA3 50- product
31.08.2023
(40/60/80).
The owner of the declaration shall be liable for the underlying information
and evidence; the IBU shall not be liable with respect to manufacturer
Valid to
information, life cycle assessment data and evidences.
30.08.2028
The EPD was created according to the specifications of EN 15804+A2. In
the following, the standard will be simplified as EN 15804.
Verification
The standard EN 15804 serves as the core PCR
Independent verification of the declaration and data according to ISO
14025:2011
internally X externally
Dipl.-Ing. Hans Peters
(Chairman of Institut Bauen und Umwelt e.V.)
Florian Pronold Mrs Kim Allbury,
(Managing Director Institut Bauen und Umwelt e.V.) (Independent verifier)
1 Environmental Product Declaration - Grundfos Holding A/S - MAGNA3 50-40/60/80 (Cast Iron)
Product
EN 300 328 V2.1.1
Product description/Product definition
The Grundfos MAGNA3 circulator pumps are designed for
circulating liquids in heating systems, air conditioning and
cooling systems and domestic hot water systems. However, the Electromagnetic Compatibility (EMC) Directive
pump range can also be used in ground source heat pump (2014/30/EU)
systems and solar heating systems.
Standards used:
EN 55014-1:2017, EN 55014-2:2015,
The MAGNA3 pump is a centrifugal pump powered by an EN 61000-3-2:2014/2019, EN 61000-6-2:2008/2019,
electrical motor. It has a high-performance neodymium magnet
rotor which increases motor efficiency and an insulation shell to EN 61000-3-3:2013 A1:2019
reduce heat loss from the cast iron pump housing with threaded
connections.
RoHS Directive 2011/65/EU and 2015/863//EU
The declaration covers three types of the MAGNA3 pump. They Standard: EN 50581:2012.
are grouped as shown below. The group reference in the
technical data and scenarios refers also to these.
Ecodesign Directive (2009/125/EC)
GROUP 1 - MAGNA 3 50-40 GROUP 2 - MAGNA 3 50-60 Commission Regulation (EC) No: 641/2009 and
GROUP 3 - MAGNA 3 50-80
Commission Regulation (EU) 622/2012
Standards used:
EN 16297-1:2012, EN 16297-2:2012, EN 16297-3:2012.
These are all the same physical products and 100 % identical
in terms of design, dimensions and materials as well as supply
chain and manufacturing processes, i.e., all cradle to gate The CE marking takes into account the proof of conformity with
processes (A1-A3). the respective harmonized norms based on the legal provisions
above.
MAGNA3 pumps are not harmonized in accordance with the
CPR.
Application
The products are also identical in terms of packaging, For the application and use the respective national
distribution, reference service life and end-of-life treatment.
provisions apply.
The only thing that differentiates the products from each other
is the software which controls how the pump operates in the The pump is designed for circulating liquids in the
system in which it is installed, making them fit for different
applications. Hence, all life cycle modules are identical, except following systems:
use stage module B6, which will change, as the applied
scenarios for electricity consumption changes. · heating systems
For the placing on the market in the European Union/European · domestic hot-water systems
Free Trade Association (EU/EFTA) (with the exception of
Switzerland) the following legal provisions apply: · air-conditioning and cooling systems
Machinery Directive (2006/42/EC) · ground-source heat-pump systems
Standard used: EN 809:1998 + A1:2009. · solar-heating systems
Radio Equipment Directive (2014/53/EU) The pump is suitable for thin, clean, non-aggressive and non-
explosive liquids, not containing solid particles or fibres that
Standards used: may attack the pump mechanically or chemically. In heating
EN 60335-1:2012/AC:2014 + A11:2014, EN 60335-2-51:2003 + systems, the water must meet the requirements of accepted
A1:2008 + A2:2012, EN 62233:2008. standards on water quality in heating systems. The pumps are
also suitable for domestic hot-water systems.
EN 55014-1:2006 + A1:2009 + A2:2011, EN 55014-1:2017, EN
61000-6-2:2005, EN 61000-3-2:2014, EN 61000-3-3:2013, Technical Data
ETSI EN 301 489-1 V2.2.0, ETSI EN 301 489-17 V3.2.0. ETSI
2 Environmental Product Declaration - Grundfos Holding A/S - MAGNA3 50-40/60/80 (Cast Iron)
The performance data of the product according to the
harmonised norms, based on the harmonisation provisions
above apply. REACH
The relevant technical specifications according to the PCR Part
B are given in the table below. This product/article/at least one partial article contains
Characteristics that are the same for all three product groups
are only given once. Others are given individually for all three substances listed in the ECHA candidate list (date:
groups.
10.06.2022) exceeding 0.1 percentage by mass: no
Constructional data
Name Value Unit
The Wahlstedt production has been assessed and certified as
Frequency 50 Hz meeting the requirements in ISO 14001, ISO 50001, ISO 45001
Voltage 230 V and ISO 9001.
Clean
Pumped liquid (e.g. water) - Reference service life
Water
No use stage scenario which refers to the lifetime of the product
Energy Efficiency Index Gr.1 0,20
is declared. However, to facilitate building calculations, an
Energy Efficiency Index Gr. 2 0,19 estimated RSL of 10 years can be used.
Energy Efficiency Index Gr. 3 0,18 This is an EU consensus-based estimation, referenced on page
Flow range Gr. 1 (max) 18,0 m3/h 37 in Appendix 7: Lot 11 – Circulators in Buildings, prepared by
AEA Energy & Environment for the European Commission in
Flow range Gr. 2 (max) 24,5 m3/h
the context of the Eco Design Directive:
Flow range Gr. 3 (max) 27,0 m3/h
Head max. Gr.1 4 m There is no definitive information on the average circulator life
Head max. Gr.2 6 m available, there is consensus within the industry that it is at
least 12 years. However, this is complicated by many factors,
Head max. Gr.3 8 m
including many being scrapped prematurely when e.g. the
Power input Gr. 1 Average (from load profile
0,067 kW boiler they are connected to is replaced.
describing use)
Power input Gr. 2 Average (from load profile
0,111 kW
describing use)
Power input Gr. 3 Average (from load profile From the estimated stock (140Mpa) and annual sales (14Mpa),
0,143 kW
describing use) the average lifetime of the circulator is taken as 10 years for the
Nominal capacity Gr.1 0,138 kW purposes of this study.
Nominal capacity Gr. 2 0,249 kW
Nominal capacity Gr. 3 0,328 kW
Performance data of the product according to the The RSL of the declared product is not directly influencing the
results in this study, as no declared use stage scenario is
harmonized standards, based on provisions for harmonization. dependent on the RSL; The use stage sub-module B6 is
declared per year as required by the PCR Part B.
Base materials/Ancillary materials
Base materials / Ancillary materials
Name Value Unit
Aluminium 16 %
Cast iron 48 %
Ceramics 0,3 %
Copper 3 %
Electronics 0,3 %
Magnet Nd 1 %
Paper 1 %
PCB 4 %
Plastics 0,4 %
Plastics, foam 1 %
Plastics GF 6 %
Rubber 0,2 %
Stainless steel 5 %
Steel 6 %
Cardboard 7 %
Plastic film 0,1 %
TOTAL 100 %
LCA: Calculation rules
The declared unit is 1 piece (pcs.) of MAGNA3 (Cast iron)
Declared Unit pump.
3 Environmental Product Declaration - Grundfos Holding A/S - MAGNA3 50-40/60/80 (Cast Iron)
transport;
Declared unit
Name Value Unit
· A1 Energy recovery and other recovery processes from
Declared unit 1 pce. secondary fuels;
Mass reference 19.87 kg/pce
Conversion factor [Mass/Declared Unit] 19.87 - · A2 Transportation up to the factory gate and internal transport;
For IBU core EPDs (where clause 3.6 is part of the EPD): for
· A3 Production of ancillary materials or pre products;
average EPDs, an estimate of the robustness of the LCA
values must be made, e.g. concerning the variability of the
· A3 Manufacturing of products and coproducts;
production process, geographical representativeness and the
influence of background data and preliminary products
· A3 Manufacturing of packaging;
compared to the environmental impacts caused by the actual
production.
· A1-A3 processing up to the end-of-waste state or disposal of
final residues.
System boundary
For secondary material inputs, the system boundary to the
previous system (providing the secondary material) is set where
outputs reach the end-of-waste state. The recycling of
System boundary
secondary material into new raw materials is included in the
system boundary of this study. Waste
materials from production processes that are recycled without
This EPD is Cradle-To-Grave. The system boundaries
any modification of the material's inherent characteristics are
modelled as closed-loop within A1-A3. This is done up to the
of the EPD follow the modular approach in EN 15804. By
input mass flow that was used during production.
decision no. 20170712-n of the SVR, the modules B3, B4 and
B5 are by default declared as "MNR" (module not relevant).
Waste for incineration arising in the product stage is accounted
for in the module where the waste is produced. The
The product stage (A1-A3) comprises raw material extraction
environmental loads from the incineration process are declared
and processing, transport processes as well as the
in the module where it occurs and the electricity and heat which
manufacturing process. The final production and assembly of
is produced from the incineration are considered as closed-loop
the MAGNA3 pump takes place at a Grundfos manufacturing
within A1-A3, as described in PCR Part A, 5.5.1. The input of
site in Germany. However, the full supply-chain leading to the
biogenic carbon from the production of packaging material is
finished product at the gate is rather complex and includes a
inventoried in A3. As required by PCR Part A, the
large amount of raw materials, components and semi-finished
corresponding end-of-life module of the packaging material, A5,
parts which come from both external suppliers as well as other
is also declared and the emissions of biogenic carbon are
Grundfos production facilities
inventoried.
The construction process stage (A4-A5) includes:
The product stage is included in the study, and according to EN
A4:
15804 the system boundary with nature is set to include those
· Transportation from factory gate to distribution centre:
processes that provide the material and energy inputs into the
system and the following manufacturing, transport up to the
· Consumption of electricity, thermal energy and water at
factory gate as well as the processing of any waste arising from
distribution centre;
those processes.
· Transportation from distribution centre to construction site;
Wastes and losses are included in the modules where they
occur according to the polluter pays principle and the modular
· Wastage during distribution.
approach of EN 15804.
A5:
· Installation process;
The product includes:
· Transport of packaging waste to the treatment site;
· A1 Extraction and processing of raw materials;
· Waste treatment of packaging.
· A1 Reuse of products or materials from a previous product
system;
The packaging material does not reach the end of waste state
but is incinerated as waste. According to European statistics,
· A1 Processing of secondary materials;
the average R1 value of incineration plants is > 0.6. Therefore,
it is assumed
· A1 Generation of electricity, steam and heat from primary
energy resources, also including their extraction, refining and
that packaging material is treated thermally in an incineration
4 Environmental Product Declaration - Grundfos Holding A/S - MAGNA3 50-40/60/80 (Cast Iron)
plant with R1 > 0.6. The loads from the combustion process of
packaging are declared in module A5 and the resulting energy
benefits in module
According to EN 15804 and the PCR Part A, the end-of-life
D, as required by the PCR Part A, 5.5.2. stage includes:
· C1 deconstruction of the product from the
Use stage (B1-B7): · building, including initial on-site sorting of the
· materials;
The use stage, related to the building fabric includes: · C2 transportation of the discarded product to a recycling site
and transportation of waste to final disposal;
· B1, use or application of the installed product;
· C3 waste processing, collection of waste fractions from the
· B2, maintenance. deconstruction and waste processing of material flows intended
for reuse, recycling and energy recovery;
The use stage related to the operation of the building
· C4 waste disposal including physical pretreatment and
includes: management of the disposal site.
· B6, operational energy use; At end of life, the MAGNA3 pump is manually disassembled
from the piping system in which it has been installed. The
· B7, operational water use. definition of the applied end-of-life scenario in this EPD follows
the requirements in the
In this study, all use stage modules are assessed, though B1,
B2 and B7 are assessed to be zero. By decision no. 20170712- PCR Part A, 6.2 regarding complex products, with a
n of the SVR, the modules B3, B4 and B5 are by default combination of recycling, thermal waste treatment and
declared as "MNR" (module landfilling. 100 % of the material is considered in the end of life
scenario as required by the PCR. An overall collection rate of
not relevant). 90 % has been assumed.
The modules include the provision and transport of all
materials, products and related energy and water use, as well
as waste processing up to the end-of-waste state or disposal of
final residues during the use stage. They also include all Materials from which energy is recovered in an incineration
impacts and process with an R1-value above 0.60 are in this study included
with the environmental burdens from the incineration process
aspects related to the losses during the use stage (i.e. inventoried in C3, the recovered energy is declared as exported
production, transport, waste processing and disposal of the lost energy in C3
products and materials).
and the energy benefits are declared in D. This procedure is
according to the PCR Part A, 5.5.6. C3 includes the mechanical
separation of the product followed by a series of sorting steps.
Generally, the geographical coverage of the datasets used Metal fractions are recycled and plastics, cardboard and
matches the actual processes taking place. Meaning, that when electronics are assumed incinerated with energy recovery. The
modelling taking place in Grundfos Bjerringbro, the Danish residual fractions are landfilled and declared in C4.
electricity grid mix is used in the model and thermal energy
from natural gas. These are generally of very high quality with The specific amounts are shown in the scenarios
very good technological, temporal and geographical
representativeness. section.
Contributions to operational energy use during the use stage Beyond system boundary (D): According to EN 15804
(B6) come from the electricity consumption of the product. The module D includes the reuse, recovery and/or recycling
annual electricity consumption is calculated by multiplying the potentials, expressed as net impacts and benefits. Any
average power input, which is based on a defined load profile, declared benefits and loads from net
with the annual running hours. For use stage (B6) European
Average electricity grid mix has been used. These values are flows leaving the product system that have not been allocated
declared in the scenarios section. as co-products and that have passed the end-of-waste state
are included in module D.
The End-of-Life stage (C1-C4) includes all activities from
when the product reaches the end of its service life and no Contributions to module D comes from waste incineration
longer provides any functionality and until all materials and processes in A5 and C3 as well as material recycling in C3. The
components are processed for specific fractions and net flows are shown in the scenarios
section.
reuse/recycling or disposed of.
5 Environmental Product Declaration - Grundfos Holding A/S - MAGNA3 50-40/60/80 (Cast Iron)
manufactured, used or handled at the end of the product´s
lifespan: Germany
Comparability
Comparability
Basically, a comparison or an evaluation of EPD data is only
possible if all the data sets to be compared were created Basically, a comparison or an evaluation of EPD data is only
according to EN 15804 and the building context, respectively possible if all the data sets to be compared were created
the product-specific characteristics of performance, are taken according to EN 15804 and the building context, respectively
into account. the product-specific characteristics of performance, are taken
into account. Software and databases used: GaBi ts
Geographic Representativeness 9.2.1.68 (database schema 8007) Ecoinvent v3.5
Land or region, in which the declared product system is
LCA: Scenarios and additional technical information
An
Characteristic product properties of biogenic carbon estimated RSL of 10 years can be used to facilitate building
The biogenic carbon content quantifies the amount of biogenic calculations. This
carbon in a construction product leaving the factory gate, and it is an EU consensus-based estimation, referenced in Appendix
will be separately declared for the product and for any 7: Lot 11 –
accompanying packaging, as required from the PCR Part A. Circulators in Buildings, prepared by AEA Energy &
The Carbon content of Cardboard and Paper is assumed to Environment for the
0.46 kg C. Overall, there is an amount of 9 weight-% Carbon in European Commission in the context of the Eco Design
the product leaving the factory gate and has to be considered Directive.
Information on describing the biogenic Carbon Content at Reference service life
factory gate
Name Value Unit
Note: 1 kg of biogenic carbon is equivalent to 44/12 kg of CO2.
Life Span according to the manufacturer 10 a
Name ValueUnit
kg Operational energy use (B6)
Biogenic carbon content in product -
C Name Value Unit
Biogenic carbon content in accompanying kg Electricity consumption Group 1 335 kWh/a
0.74
packaging C Electricity consumption Group 2 555 kWh/a
Electricity consumption Group 3 715 kWh/a
The following technical scenario information is required for the Average power input, Group 1 0,067 kW
declared modules and optional for non-declared modules.
Average power input, Group 2 0,111 kW
Modules for which no information is declared can be deleted;
Average power input, Group 3 0,143 kW
additional information can also be listed if necessary.
Running hours (all groups) 5.000 h/a
The following technical information is a basis for the declared
End of life (C1-C4)
modules or can be used for developing specific scenarios in the
context of a building assessment if modules are not declared Name Value Unit
(MND). Collected as mixed construction waste 18,24 kg
Transportation distance (C2) 500 km
A5 is not declared including the disposal of the packaging
Aluminium for recycling 2,8 kg
material on the construction site, the amounts of packaging
Steel for recycling 9,5 kg
materials included in the LCA calculations must be declared as
technical scenario information for Module A5. Copper for recycling 0,51 kg
Stainless steel for recycling 0,91 kg
Plastics for incineration w/energy 1,33 kg
Transport from the gate to the site (A4) Electronics for incineration w/energy 0,81 kg
Name Value Unit Landfilling 2,38 kg
Litres of fuel 0,052 l/100km
Reuse, recovery and/or recycling potentials (D), relevant
Transport distance 2003 km
scenario information
Capacity utilisation (including empty runs) 85 %
Name Value Unit
Gross density of products transported 383 kg/m3
A5, incineration w/energy recov. (LDPE foil) 3,6 MJ
Wastage during distribution 0,02 %
A5, incineration w/energy recov.
6,53 MJ
(Paper/Cardboard)
Installation into the building (A5)
C3, steel for recycling (net amounts) -1,2 kg
Name ValueUnit
C3, stainless steel for recycling (net amounts) 0,52 kg
Packaging waste for incineration (LDPE film) 0,031 kg
C3, aluminium for recycling (net amounts) -0,383 kg
Packaging waste for incineration
(Paper/Cardboard) 1,6 kg C3, copper for recycling (net amounts) 0,221 kg
C3, plastics for incineration, w/ energy recov. 1,33 kg
C3, electronics for incineration, w/ energy recov. 0,814 kg
6 Environmental Product Declaration - Grundfos Holding A/S - MAGNA3 50-40/60/80 (Cast Iron)
LCA: Results
Characterization model: EN 15804 - 2012+A2 - 2019, PEF. By Decision no. 20170712-n of the IBU SVR, the modules B3, B4, B5 are
marked as MNR (module not relevant) as default. The LCA results in module B6 are given on a period of one year, according to PCR
Part B. To obtain the results from module B6 over the entire life cycle, the LCA results of module B6 must be multiplied by the
estimated RSL of 10 years. The indicator results for module B6 are declared for Group 1. B6 indicator results for other groups can be
derived by multiplying the B6 indicator results with the following factors:
Group 2: 1,64
Group 3: 2,12
DESCRIPTION OF THE SYSTEM BOUNDARY (X = INCLUDED IN LCA; ND = MODULE OR INDICATOR NOT DECLARED; MNR =
MODULE NOT RELEVANT)
Benefits and
Construction loads beyond
Product stage Use stage End-of-life stage
process stage the system
boundaries
la ire ta m w a Ry lp p u s tro p s n a rT g n iru tc a fu n a M e h t m o rf tro p s n a rTe tis e h t o t e ta g y lb m e s s A e s U e c n a n e tn ia M ria p e R tn e m e c a lp e R tn e m h s ib ru fe R y g re n e la n o ita re p Oe s u re ta w la n o ita re p Oe s u n o itc u rts n o c -e Dn o itilo m e d tro p s n a rT g n is s e c o rp e ts a W la s o p s iD -e s u e R-y re v o c e R-g n ilc y c e Rla itn e to p
A1 A2 A3 A4 A5 B1 B2 B3 B4 B5 B6 B7 C1 C2 C3 C4 D
X X X X X MND MND MNR MNR MNR X MND X X X X X
RESULTS OF THE LCA - ENVIRONMENTAL IMPACT according to EN 15804+A2: 1PCS of MAGNA3 50-40/60/80 (Cast Iron)
Parameter Unit A1 A2 A3 A4 A5 B6 C1 C2 C3 C4 D
GWP-total kg CO 2 eq 9.65E+01 1.24E+00 1.14E+00 1.24E+00 2.35E+00 1.36E+02 0 5.08E-01 6.11E+00 1.21E-01 -1.07E-01
GWP-fossil kg CO 2 eq 9.6E+01 1.24E+00 3.75E+00 1.24E+00 1.39E-01 1.35E+02 0 5.05E-01 6.1E+00 1.25E-01 -1.02E-01
GWP-
biogenic kg CO 2 eq 3.48E-01 -1.62E-03 -2.65E+00 -2.5E-03 2.21E+00 4.5E-01 0 -8.52E-04 5.46E-03 -3.76E-03 -2.47E-03
GWP-luluc kg CO 2 eq 1.51E-01 8.79E-03 3.43E-02 9.77E-03 8E-05 1.95E-01 0 4.11E-03 2.73E-03 1.1E-04 -2.57E-03
kg CFC11
ODP 9.27E-08 2.14E-16 4.06E-09 1.93E-11 4.32E-16 2.97E-12 0 9.31E-17 4.1E-14 2.81E-16 -7.57E-13
eq
AP mol H+ eq 5.42E-01 9.94E-03 1.63E-02 7.19E-03 6.75E-04 2.98E-01 0 2.98E-03 4.82E-03 3.88E-04 -1.12E-02
EP-
kg P eq 1.6E-03 3.34E-06 5.6E-05 4.01E-06 9.88E-08 3.6E-04 0 1.54E-06 7.22E-06 1.36E-05 -4.05E-06
freshwater
EP-marine kg N eq 6.78E-02 3.35E-03 2.98E-03 3.43E-03 2.46E-04 6.61E-02 0 1.44E-03 1.18E-03 8.95E-05 -3.88E-04
EP-terrestrial mol N eq 7.12E-01 3.7E-02 2.99E-02 3.8E-02 3.06E-03 6.95E-01 0 1.59E-02 1.33E-02 9.81E-04 -3.78E-03
kg NMVOC
POCP 2.1E-01 7.85E-03 8.68E-03 6.53E-03 6.43E-04 1.81E-01 0 2.73E-03 3.22E-03 2.88E-04 -1.32E-03
eq
ADPE kg Sb eq 1.31E+03 1.63E+01 5.21E+01 1.66E+01 8.12E-01 2.37E+03 0 6.77E+00 3.35E+01 1.79E+00 -1.62E+01
ADPF MJ 5.58E-03 9.17E-08 5.95E-05 1.23E-06 7.19E-09 3.9E-05 0 4.1E-08 5.4E-07 8.44E-09 -6.17E-04
m3 world eq
WDP 2.55E+01 1.09E-02 1.49E-01 1.79E-02 2.89E-01 2.94E+01 0 4.95E-03 8.4E-01 -1.38E-03 -3.84E-01
deprived
GWP = Global warming potential; ODP = Depletion potential of the stratospheric ozone layer; AP = Acidification potential of land and water; EP =
Eutrophication potential; POCP = Formation potential of tropospheric ozone photochemical oxidants; ADPE = Abiotic depletion potential for non-fossil
resources; ADPF = Abiotic depletion potential for fossil resources; WDP = Water (user) deprivation potential)
RESULTS OF THE LCA - INDICATORS TO DESCRIBE RESOURCE USE according to EN 15804+A2: 1PCS of MAGNA3 50-
40/60/80 (Cast Iron)
Parameter Unit A1 A2 A3 A4 A5 B6 C1 C2 C3 C4 D
PERE MJ 3.5E+02 8.43E-01 4.31E+01 1.04E+00 1.4E-01 1.05E+03 0 3.91E-01 1.45E+01 1.26E-01 5.28E+00
PERM MJ 0 0 0 0 0 0 0 0 0 0 0
PERT MJ 3.5E+02 8.43E-01 4.31E+01 1.04E+00 1.4E-01 1.05E+03 0 3.91E-01 1.45E+01 1.26E-01 5.28E+00
PENRE MJ 1.31E+03 1.64E+01 5.21E+01 1.67E+01 8.13E-01 2.37E+03 0 6.79E+00 3.35E+01 1.79E+00 -1.61E+01
PENRM MJ 0 0 0 0 0 0 0 0 0 0 0
PENRT MJ 1.31E+03 1.64E+01 5.21E+01 1.67E+01 8.13E-01 2.37E+03 0 6.79E+00 3.35E+01 1.79E+00 -1.61E+01
SM kg 1.47E+01 0 2.31E-01 2.99E-03 0 0 0 0 0 0 0
RSF MJ 1.46E-23 0 0 2.91E-27 0 0 0 0 0 0 0
NRSF MJ 1.71E-22 0 0 3.42E-26 0 0 0 0 0 0 0
FW m3 7.8E-01 9.87E-04 2.14E-02 1.29E-03 6.82E-03 1.21E+00 0 4.56E-04 2.69E-02 2.28E-05 2.62E-02
PERE = Use of renewable primary energy excluding renewable primary energy resources used as raw materials; PERM = Use of renewable primary
energy resources used as raw materials; PERT = Total use of renewable primary energy resources; PENRE = Use of non-renewable primary energy
excluding non-renewable primary energy resources used as raw materials; PENRM = Use of non-renewable primary energy resources used as raw
materials; PENRT = Total use of non-renewable primary energy resources; SM = Use of secondary material; RSF = Use of renewable secondary fuels;
NRSF = Use of non-renewable secondary fuels; FW = Use of net fresh water
RESULTS OF THE LCA – WASTE CATEGORIES AND OUTPUT FLOWS according to EN 15804+A2:
1PCS of MAGNA3 50-40/60/80 (Cast Iron)
7 Environmental Product Declaration - Grundfos Holding A/S - MAGNA3 50-40/60/80 (Cast Iron)
Parameter Unit A1 A2 A3 A4 A5 B6 C1 C2 C3 C4 D
HWD kg 2.54E-04 6.72E-07 1.22E-04 8.19E-07 4.21E-09 9.81E-07 0 3.14E-07 1.72E-08 7.18E-09 -3.23E-04
NHWD kg 4.02E+00 2.49E-03 2.81E-01 3.16E-03 7.86E-02 1.68E+00 0 1.08E-03 5.73E-01 2.05E+00 1.45E+00
RWD kg 5.46E-02 2.89E-05 1.44E-03 4.53E-05 3.9E-05 3.6E-01 0 1.25E-05 4.95E-03 2.14E-05 -1.38E-03
CRU kg 0 0 0 0 0 0 0 0 0 0 0
MFR kg 0 0 0 0 0 0 0 0 1.37E+01 0 0
MER kg 0 0 0 0 0 0 0 0 0 0 0
EEE MJ 0 0 0 0 3.6E+00 0 0 0 7.14E+00 0 0
EET MJ 0 0 0 0 6.53E+00 0 0 0 1.29E+01 0 0
HWD = Hazardous waste disposed; NHWD = Non-hazardous waste disposed; RWD = Radioactive waste disposed; CRU = Components for re-use;
MFR = Materials for recycling; MER = Materials for energy recovery; EEE = Exported electrical energy; EET = Exported thermal energy
RESULTS OF THE LCA – additional impact categories according to EN 15804+A2-optional:
1PCS of MAGNA3 50-40/60/80 (Cast Iron)
Parameter Unit A1 A2 A3 A4 A5 B6 C1 C2 C3 C4 D
Disease
PM 6.51E-06 1.22E-07 2.28E-07 4.28E-08 3.83E-09 2.5E-06 0 1.75E-08 4.09E-08 3.95E-09 -2.78E-07
incidence
IR kBq U235 eq 6.02E+00 4.25E-03 2.26E-01 6.33E-03 6E-03 5.9E+01 0 1.85E-03 8.12E-01 3.04E-03 -9.35E-02
ETP-fw CTUe 8E+02 1.22E+01 1.73E+01 1.22E+01 4.11E-01 1.01E+03 0 5.06E+00 1.46E+01 1.26E+00 -5.66E+00
HTP-c CTUh 1.64E-06 2.49E-10 6.46E-07 7.09E-10 2.02E-11 2.8E-08 0 1.05E-10 4.49E-10 7.23E-11 -6.74E-08
HTP-nc CTUh 2.38E-06 1.35E-08 5.33E-08 1.48E-08 9.63E-10 1.03E-06 0 6.01E-09 1.82E-08 6.31E-09 -2.85E-09
SQP SQP 3.69E+02 5.09E+00 7.98E+01 5.75E+00 2.21E-01 7.55E+02 0 2.38E+00 1.06E+01 1.29E-01 -1.5E+01
PM = Potential incidence of disease due to PM emissions; IR = Potential Human exposure efficiency relative to U235; ETP-fw = Potential comparative
Toxic Unit for ecosystems; HTP-c = Potential comparative Toxic Unit for humans (cancerogenic); HTP-nc = Potential comparative Toxic Unit for humans
(not cancerogenic); SQP = Potential soil quality index
Disclaimer 1 – for the indicator 'Potential Human exposure efficiency relative to U235'. This impact category deals mainly with the
eventual impact of low-dose ionizing radiation on human health of the nuclear fuel cycle. It does not consider effects due to possible
nuclear accidents, occupational exposure or radioactive waste disposal in underground facilities. Potential ionizing radiation from the
soil, from radon and from some construction materials is also not measured by this indicator. Disclaimer 2 – for the indicators 'abiotic
depletion potential for non-fossil resources', 'abiotic depletion potential for fossil resources', 'water (user) deprivation potential,
deprivation-weighted water consumption', 'potential comparative toxic unit for ecosystems', 'potential comparative toxic unit for humans
– cancerogenic', 'Potential comparative toxic unit for humans - not cancerogenic', 'potential soil quality index'. The results of this
environmental impact indicator shall be used with care as the uncertainties on these results are high as there is limited experience with
the indicator.
Disclaimer 3: JRC Technical Reports, Version 2, 2018 Page 6, for the indicator "EP-freshwater". This indicator has been calculated as
'kg P eq' as required in the characterization model EUTREND model, Struijs et al., 2009b, as implemented in ReCiPe;
References
Standards
States relating to electromagnetic compatibility
Machinery Directive
DIRECTIVE 2006/42/EC OF THE EUROPEAN
Ecodesign Directive
PARLIAMENT AND OF THE COUNCIL of 17 May
DIRECTIVE 2009/125/EC OF THE EUROPEAN
2006 on machinery
PARLIAMENT AND OF THE COUNCIL of 21 October
2009 establishing a framework for the setting of
Radio Equipment Directive
ecodesign requirements for energy-related products
DIRECTIVE 2014/53/EU OF THE EUROPEAN PARLIAMENT
AND OF THE COUNCIL of 16 April 2014 on the harmonization
of the laws of the Member States relating to the making
available on the market of EC 641/2009
radio equipment COMMISSION REGULATION (EC) No 641/2009 of 22 July
2009 implementing Directive 2005/32/EC of the European
Parliament and of the Council with regard to ecodesign
requirements for glandless standalone circulators and
Electromagnetic Compatibility (EMC) Directive glandless circulators integrated in
DIRECTIVE 2014/30/EU OF THE EUROPEAN products
PARLIAMENT AND OF THE COUNCIL of 26 February
2014 on the harmonization of the laws of the Member EC 622/2012
8 Environmental Product Declaration - Grundfos Holding A/S - MAGNA3 50-40/60/80 (Cast Iron)
EN 55014-1:2017, Electromagnetic compatibility –
COMMISSION REGULATION (EU) No 622/2012 of 11 July Requirements for household appliances, electric tools and
2012 amending Regulation (EC) No 641/2009 with regard to similar apparatus – Part 1: Emission
ecodesign requirements for glandless standalone circulators
and glandless circulators integrated in products
EN 55014-2
DIRECTIVE 2011/65/EU EN 55014-2:2015, Electromagnetic compatibility –
DIRECTIVE 2011/65/EU OF THE EUROPEAN Requirements for household appliances, electric tools
PARLIAMENT AND OF THE COUNCIL of 8 June 2011 and similar apparatus – Part 2: Immunity – Product
on the restriction of the use of certain hazardous family standard (CISPR 14-2:2015)
substances in electrical and electronic equipment
EN 50581:2012
DIRECTIVE 2015/863/EU EN 50581:2012, Technical documentation for the
DIRECTIVE 2015/863/EU of 31 March 2015 amending assessment of electrical and electronic products with
Annex II to Directive 2011/65/EU of the European respect to the restriction of hazardous substances
Parliament and of the Council as regards the list of
restricted substances EN 60335-1
EN 60335-1:2012/A11:2014/A13:2017, Household
ETSI EN 301 489-1 and similar electrical appliances – Safety – Part 1:General
requirements
ETSI EN 301 489-1 V2.2.0, Electromagnetic Compatibility
(EMC) standard for radio equipment and services; Part 1:
Common technical requirements
EN 60335-2-51
EN 60335-2-51:2003-03 + A1:2008 + A2:2012, Household and
ETSI EN 301 489-17 similar electrical appliances – Safety –Part 2-51: Particular
requirements for stationary circulation pumps for heating and
ETSI EN 301 489-17 V3.2.0, Electromagnetic Compatibility service water installations
(EMC) standard for radio equipment and services; Part 17:
Specific conditions for Broadband Data Transmission Systems
EN 61000-3-2
EN 61000-3-2:2014/2019, Electromagnetic compatibility (EMC)
– Part 3-2: Limits – Limits for harmonic current emissions
(equipment input current =16 A per phase)
ETSI EN 300 328 V2.1.1
ETSI EN 300 328 V2.1.1, Wideband transmission systems; EN 61000-3-3
Data transmission equipment operating in the 2,4 GHz ISM
band and using wide band modulation techniques EN 61000-3-3:2013-08/ A1:2019, Electromagnetic compatibility
(EMC) – Part 3-3:
Limits – Limitation of voltage changes, voltage fluctuations and
flicker in public low voltage supply systems, for equipment with
EN 809
rated current <= 16 A per phase and not subject to conditional
EN 809:1998-10 + A1:2009, Pumps and pump units for connection
liquids - Common safety requirements
EN 61000-6-2
EN 55014-1 EN 61000-6-2:2008/2019, Electromagnetic compatibility (EMC)
– Part 6-2: Generic standards –Immunity for industrial
9 Environmental Product Declaration - Grundfos Holding A/S - MAGNA3 50-40/60/80 (Cast Iron)
environments PCR Part B
Institut Bauen und Umwelt e.V., Berlin (pub.): Product Category
Rules for Building-Related Products and Services, Product
EN 16297-1 Category Rules for Construction Products from the range of
Environmental Product Declarations of Institut Bauen und
EN 16297-1:2012-10, Pumps – Rotodynamic pumps – Umwelt (IBU), Part B: Requirements on the EPD for Pumps for
Glandless circulators – Part 1: liquids and liquids with solids, Version 1.0 (2018)
General requirements and procedures for testing and
calculation of energy efficiency index (EEI)
Further references
EN 16297-2
EN 16297-2:2012-10, Pumps – Rotodynamic pumps – CPR
Glandless circulators – Part 2: Calculation of energy efficiency
index (EEI) for standalone circulators REGULATION (EU) No 305/2011 OF THE EUROPEAN
PARLIAMENT AND OF THE COUNCIL of 9 March 2011 laying
down harmonised conditions for the marketing of construction
products and repealing Council Directive 89/106/EEC
EN 16297-3
EN 16297-3:2012, Pumps – Rotodynamic pumps –Glandless
circulators – Part 3: Energy efficiency index (EEI) for circulators CML 2001
integrated in products
Impact assessment characterization factors Institute of
Environmental Sciences, Leiden University, Netherlands
ISO 14001
EN ISO 14001:2015-09, Environmental management systems - ECHA candidate list
Requirements with guidance for use
Candidate List of substances of very high concern (SVHCs) for
authorisation, European Chemicals Agency (ECHA), Helsinki,
Finland
ISO 14025
DIN EN /ISO 14025:2011-10, Environmental labels and
declarations — Type III environmental declarations — Ecoinvent
Principles and procedures
Ecoinvent v3.5
EN 15804
GaBi ts
EN 15804:2012-04+A1 2013, Sustainability of construction
works — Environmental Product Declarations — Core rules for GaBi ts 9.2.1.68 (database schema 8007)
the product category of construction products
REACH
PCR Part A
Regulation (EC) No 1907/2006 of the European Parliament and
Institut Bauen und Umwelt e.V., Berlin (pub.): Product Category of the Council of 18 December 2006 concerning the
Rules for Building-Related Products and Services, Product Registration, Evaluation, Authorisation and Restriction of
Category Rules for Construction Products from the range of Chemicals (REACH) (Status: 27.06.2018)
Environmental Product Declarations of Institut Bauen und
Umwelt (IBU), Part A: Calculation Rules for the Life Cycle
Assessment and Requirements on the Project Report, Version
1.7 (2021) SVR
Advisory Board (formerly SVA)
10 Environmental Product Declaration - Grundfos Holding A/S - MAGNA3 50-40/60/80 (Cast Iron)
Decision no. The literature referred to in the Environmental Product
20170712-n Declaration must be listed in full.Standards already fully quoted
in the EPD do not need to be listed here again.
The current version of PCR Part A and PCR Part B of the PCR
document on which they are based must be referenced.
11 Environmental Product Declaration - Grundfos Holding A/S - MAGNA3 50-40/60/80 (Cast Iron)
Publisher
Institut Bauen und Umwelt e.V. +49 (0)30 3087748- 0
Hegelplatz 1 info@ibu-epd.com
10117 Berlin www.ibu-epd.com
Germany
Programme holder
Institut Bauen und Umwelt e.V. +49 (0)30 3087748- 0
Hegelplatz 1 info@ibu-epd.com
10117 Berlin www.ibu-epd.com
Germany
Author of the Life Cycle Assessment
Grundfos Holding A/S +45 87501400
Poul Due Jensens Vej 7 atomic@grundfos.com
8850 Bjerringbro www.grundfos.com
Denmark
Owner of the Declaration
Grundfos Holding A/S +45 87501400
Poul Due Jensens Vej 7 atomic@grundfos.com
8850 Bjerringbro www.grundfos.com
Denmark
12 Environmental Product Declaration - Grundfos Holding A/S - MAGNA3 50-40/60/80 (Cast Iron)
