ENVIRONMENTAL PRODUCT DECLARATION
as per ISO 14025 and EN 15804+A2
Owner of the Declaration Grundfos Holding A/S
Publisher Institut Bauen und Umwelt e.V. (IBU)
Programme holder Institut Bauen und Umwelt e.V. (IBU)
Declaration number EPD-GRU-20240018-CBA5-EN
Issue date 18/07/2024
Valid to 16/06/2029
MAGNA3 50-40/60/80/100/120 F (Stainless Steel) and MAGNA3 32-
120 F (Stainless Steel)
Grundfos Holding A/S
www.ibu-epd.com | https://epd-online.com
General Information
Grundfos Holding A/S MAGNA3 50-40/60/80/100/120 F (Stainless Steel)
and MAGNA3 32-120 F (Stainless Steel)
Programme holder Owner of the declaration
IBU – Institut Bauen und Umwelt e.V. Grundfos Holding A/S
Hegelplatz 1 Poul Due Jensens Vej 7
10117 Berlin 8850 Bjerringbro
Germany Denmark
Declaration number Declared product / declared unit
EPD-GRU-20240018-CBA5-EN 1 PCS. of MAGNA3 50-40/60/80/100/120 F (Stainless Steel) / 1 PCS. of
MAGNA3 32-120 F (Stainless Steel)
This declaration is based on the product category rules: Scope:
Pumps for liquids and liquids with solids, 01/08/2021 The declaration applies to 1 piece of MAGNA3 Stainless Steel pump.
(PCR checked and approved by the SVR)
The product is produced in Wahlstedt, Germany, and the life cycle
assessment is based on data collected at the production site. Production
Issue date has been modeled using annual production data from 2021-2022. The
declaration covers six different types of the MAGNA3 50-40/60/80/100/120
18/07/2024
F and MAGNA3 32-120 F (flanged version).
The owner of the declaration shall be liable for the underlying information
and evidence; the IBU shall not be liable with respect to manufacturer
Valid to
information, life cycle assessment data and evidences.
16/06/2029
The EPD was created according to the specifications of EN 15804+A2. In
the following, the standard will be simplified as EN 15804.
Verification
The standard EN 15804 serves as the core PCR
Independent verification of the declaration and data according to ISO
14025:2011
internally X externally
Dipl.-Ing. Hans Peters
(Chairman of Institut Bauen und Umwelt e.V.)
Florian Pronold Mrs Kim Allbury,
(Managing Director Institut Bauen und Umwelt e.V.) (Independent verifier)
1 Environmental Product Declaration - Grundfos Holding A/S - MAGNA3 50-40/60/80/100/120 F (Stainless Steel) and MAGNA3 32-120 F (Stainless Steel)
Product
Product description/Product definition Electromagnetic Compatibility (EMC) Directive
The Grundfos MAGNA3 circulator pumps are designed for (2014/30/EU)
circulating liquids in heating systems, air conditioning and
cooling systems and domestic hot water systems. However, the Standards used:
pump range can also be used in ground source heat pump EN 55014-1:2017, EN 55014-2:2015,
systems and solar heating systems.
EN 61000-3-2:2014/2019, EN 61000-6-2:2008/2019,
The MAGNA3 pump is a centrifugal pump powered by an
electrical motor. It has a high-performance neodymium magnet EN 61000-3-3:2013 A1:2019
rotor which increases motor efficiency and an insulation shell to
reduce heat loss from the cast iron pump housing with threaded RoHS Directive 2011/65/EU and 2015/863//EU
connections.
Standard: EN 50581:2012.
The declaration covers six types of the MAGNA3 pump. They
are listed below. The group reference in the technical data and Ecodesign Directive (2009/125/EC)
scenarios refers also to these.
Commission Regulation (EC) No: 641/2009 and
MAGNA3 50-40 F (Group 1)
MAGNA3 50-60 F (Group 2) Commission Regulation (EU) 622/2012
MAGNA3 50-80 F (Group 3)
MAGNA3 50-100 F (Group 4) Standards used:
MAGNA3 50-120 F (Group 5) EN 16297-1:2012, EN 16297-2:2012, EN 16297-3:2012.
MAGNA3 32-120 F (Group 6)
The CE marking takes into account the proof of conformity with
The MAGNA 3 50-40/60/80/100/120 F are all the same physical the respective harmonised norms based on the legal provisions
products and 100 % identical in terms of design, dimensions above.
and materials as well as supply chain and manufacturing MAGNA3 pumps are not harmonised in accordance with the
processes, i.e., all cradle to gate processes (A1-A3).The CPR.
MAGNA 3 32-120 flanged version (F), although smaller, utilizes
the same technology and materials as the MAGNA 3 50- Application
40/60/80/100/120 F. Given its smaller size, it is expected to For the application and use the respective national provisions
have a lower environmental impact in A1-A3, but the MAGNA 3 apply.
50-40/60/80/100/120 F results will cover it being the 'worst-
case' scenario EPD of the MAGNA3 32-120 F. The justification The pump is designed for circulating liquids in the following
is the reduced material usage and the lower energy systems:
consumption during operation. The technical specifications
table is separate for the 32-120 F, which clearly proves the · heating systems
justification. The B6 factor will also be indicated.
The products are also identical in terms of packaging, · domestic hot-water systems
distribution, reference service life and end-of-life treatment.
· air-conditioning and cooling systems
The only thing that differentiates the products from each other
is the software which controls how the pump operates in the · ground-source heat-pump systems
system in which it is installed, making them fit for different
applications. Hence, all life cycle modules are identical, except · solar-heating systems
use stage module B6, which will change, as the applied
scenarios for electricity consumption changes. The pump is suitable for thin, clean, non-aggressive and non-
explosive liquids, not containing solid particles or fibres that
For the placing on the market in the European Union/European may attack the pump mechanically or chemically. In heating
Free Trade Association (EU/EFTA) (with the exception of systems, the water must meet the requirements of accepted
Switzerland) the following legal provisions apply: standards on water quality. The pumps are also suitable for
domestic hot-water systems.
Machinery Directive (2006/42/EC)
Technical Data
Standard used: EN 809:1998 + A1:2009. The performance data of the product according to the
harmonised norms, based on the harmonisation provisions
Radio Equipment Directive (2014/53/EU) above apply.
The relevant technical specifications according to the PCR Part
Standards used: B are given in the table below.
EN 60335-1:2012/AC:2014 + A11:2014, EN 60335-2-51:2003 + Characteristics that are the same for all three product groups
A1:2008 + A2:2012, EN 62233:2008. are only given once. Others are given individually for all three
groups.
EN 55014-1:2006 + A1:2009 + A2:2011, EN 55014-1:2017, EN Constructional data
61000-6-2:2005, EN 61000-3-2:2014, EN 61000-3-3:2013,
ETSI EN 301 489-1 V2.2.0, ETSI EN 301 489-17 V3.2.0. ETSI
EN 300 328 V2.1.1
2 Environmental Product Declaration - Grundfos Holding A/S - MAGNA3 50-40/60/80/100/120 F (Stainless Steel) and MAGNA3 32-120 F (Stainless Steel)
Name Value Unit Name Value Unit
Frequency 50 Hz Aluminium 15,11 %
Voltage 230 V Ceramics 0,34 %
Clean Copper 2,85 %
Pumped liquid (e.g. water) -
Water Electronics 0,3 %
Energy Efficiency Index 50-40 F 0,20 Magnet Nd 1,22 %
Energy Efficiency Index 50-60 F 0,19 Paper 0,56 %
Energy Efficiency Index 50-80 F 0,18 PCB 4,19 %
Energy Efficiency Index 50-100 F 0,18 Plastics 0,37 %
Energy Efficiency Index 50-120 F 0,17 Plastics, foam 0,96 %
Energy Efficiency Index 32-120 F 0,18 Plastics GF 5,88 %
Flow range 50-40 F (max) 18,0 m3/h Rubber 0,19 %
Flow range 50-60 F (max) 24,5 m3/h Stainless steel 55,07 %
Flow range 50-80 F (max) 27,0 m3/h Steel 5,68 %
Flow range 50-100 F (max) 32 m3/h Cardboard 7,23 %
Flow range 50-120 F (max) 34,8 m3/h Plastic film 0,08 %
Flow range 32-120 F (max) 21,1 m3/h TOTAL 100 %
Head max. 50-40 F 4 m REACH
Head max. 50-60 F 6 m
This product/article/at least one partial article contains
Head max. 50-80 F 8 m
substances listed in the ECHA candidate list (date:10.06.2022)
Head max. 50-100 F 10 m
exceeding 0.1 percentage by mass: no
Head max 50-120 F 12 m The Wahlstedt production has been assessed and certified as
Head max 32-120 F 12 m meeting the requirements in ISO 14001, ISO 50001, ISO 45001
Power input 50-40 F Average (from load profile and ISO 9001.
0,067 kW
describing use)
Reference service life
Power input 50-60 F Average (from load profile
0,111 kW No use stage scenario which refers to the lifetime of the product
describing use)
is declared. However, to facilitate building calculations, an
Power input 50-80 F Average (from load profile estimated RSL of 10 years can be used.
0,143 kW
describing use) This is an EU consensus-based estimation, referenced on page
Power input 50-100 F Average (from load 37 in Appendix 7: Lot 11 – Circulators in Buildings, prepared by
0,184 kW
profile describing use) AEA Energy & Environment for the European Commission in
Power input 50-120 F Average (from load the context of the Eco Design Directive:
0,228 kW
profile describing use)
There is no definitive information on the average circulator life
Power input 32-120 F Average (from load
0,152 kW available, there is consensus within the industry that it is at
profile describing use)
least 12 years. However, this is complicated by many factors,
Nominal capacity 50-40 F 0,138 kW
including many being scrapped prematurely when e.g. the
Nominal capacity 50-60 F 0,249 kW boiler they are connected to is replaced.
Nominal capacity 50-80 F 0,328 kW
Nominal capacity 50-100 F 0,403 kW From the estimated stock (140Mpa) and annual sales (14Mpa),
the average lifetime of the circulator is taken as 10 years for the
Nominal capacity 50-120 F 0,498 kW
purposes of this study.
Nominal capacity 32-120 F 0,333 kW
Performance data of the product according to the harmonised The RSL of the declared product is not directly influencing the
standards, based on provisions for harmonisation. results in this study, as no declared use stage scenario is
dependent on the RSL; The use stage sub-module B6 is
Base materials/Ancillary materials declared per year as required by the PCR Part B.
Base materials / Ancillary materials
LCA: Calculation rules
Name Value Unit
Declared Unit
Declared unit 1 pce.
The declared unit is 1 piece (pcs.) of MAGNA3 Stainless Steel
Mass reference 50-40/60/80/100/120 F 20.55 kg/pce
pump.
Conversion factor [Mass/Declared Unit] 50-
Declared unit 20.55 -
40/60/80/100/120 F
Mass reference 32-120 F 17.4 kg/piece
Conversion factor [Mass/Declared Unit] 32-120
17.4
F
Other declared units are allowed if the conversion is shown
transparently.
3 Environmental Product Declaration - Grundfos Holding A/S - MAGNA3 50-40/60/80/100/120 F (Stainless Steel) and MAGNA3 32-120 F (Stainless Steel)
Waste for incineration arising in the product stage is accounted
System boundary for in the module where the waste is produced. The
System boundary environmental loads from the incineration process are declared
in the module where it occurs and the electricity and heat which
is produced from the incineration are considered as closed-loop
This EPD is Cradle-To-Grave. The system boundaries within A1-A3, as described in PCR Part A, 5.5.1. The input of
biogenic carbon from the production of packaging material is
of the EPD follow the modular approach in EN 15804. By inventoried in A3. As required by PCR Part A, the
decision no. 20170712-n of the SVR, the modules B3, B4 and corresponding end-of-life module of the packaging material, A5,
B5 are by default declared as "MNR" (module not relevant). is also declared and the emissions of biogenic carbon are
inventoried.
The product stage (A1-A3) comprises raw material extraction
and processing, transport processes as well as the The construction process stage (A4-A5) includes:
manufacturing process. The final production and assembly of
the MAGNA3 pump takes place at a Grundfos manufacturing A4:
site in Germany. However, the full supply-chain leading to the
finished product at the gate is rather complex and includes a · Transportation from factory gate to the distribution centre:
large amount of raw materials, components and semi-finished
parts which come from both external suppliers as well as other · Consumption of electricity, thermal energy and water at the
Grundfos production facilities distribution centre;
The product stage is included in the study, and according to EN · Transportation from distribution centre to construction site;
15804 the system boundary with nature is set to include those
processes that provide the material and energy inputs into the · Wastage during distribution.
system and the following manufacturing, transport up to the
factory gate as well as the processing of any waste arising from A5:
those processes.
· Installation process;
Wastes and losses are included in the modules where they
occur according to the polluter pays principle and the modular · Transport of packaging waste to the treatment site;
approach of EN 15804.
· Waste treatment of packaging.
The product includes:
The packaging material does not reach the end of waste state
· A1 Extraction and processing of raw materials; but is incinerated as waste. According to European statistics,
the average R1 value of incineration plants is > 0.6. Therefore,
· A1 Reuse of products or materials from a previous product it is assumed that packaging material is treated thermally in an
system; incineration plant with R1 > 0.6. The loads from the combustion
process of packaging are declared in module A5 and the
· A1 Processing of secondary materials; resulting energy benefits in module D, as required by the PCR
Part A, 5.5.2.
· A1 Generation of electricity, steam and heat from primary
energy resources, also including their extraction, refining and Use stage (B1-B7):
transport;
The use stage, related to the building fabric includes:
· A1 Energy recovery and other recovery processes from
secondary fuels; · B1, use or application of the installed product;
· A2 Transportation up to the factory gate and internal transport; · B2, maintenance.
· A3 Production of ancillary materials or pre products; The use stage related to the operation of the building includes:
· A3 Manufacturing of products and coproducts; · B6, operational energy use;
· A3 Manufacturing of packaging; · B7, operational water use.
· A1-A3 processing up to the end-of-waste state or disposal of In this study, all use stage modules are assessed, though B1,
final residues. B2 and B7 are assessed to be zero. By decision no. 20170712-
n of the SVR, the modules B3, B4 and B5 are by default
For secondary material inputs, the system boundary to the declared as "MNR" (module not relevant).
previous system (providing the secondary material) is set where The modules include the provision and transport of all
outputs reach the end-of-waste state. The recycling of materials, products and related energy and water use, as well
secondary material into new raw materials is included in the as waste processing up to the end-of-waste state or disposal of
system boundary of this study. Waste final residues during the use stage. They also include all
impacts and aspects related to the losses during the use stage
materials from production processes that are recycled without (i.e. production, transport, waste processing and disposal of the
any modification of the material's inherent characteristics are lost products and materials).
modelled as closed-loop within A1-A3. This is done up to the
input mass flow that was used during production. Generally, the geographical coverage of the datasets used
matches the actual processes taking place. Meaning, that when
4 Environmental Product Declaration - Grundfos Holding A/S - MAGNA3 50-40/60/80/100/120 F (Stainless Steel) and MAGNA3 32-120 F (Stainless Steel)
modelling taking place in Grundfos Bjerringbro, the Danish with the environmental burdens from the incineration process
electricity grid mix is used in the model and thermal energy inventoried in C3, the recovered energy is declared as exported
from natural gas. These are generally of very high quality with energy in C3 and the energy benefits are declared in D. This
very good technological, temporal and geographical procedure is according to the PCR Part A, 5.5.6. C3 includes
representativeness. the mechanical separation of the product followed by a series
of sorting steps. Metal fractions are recycled and plastics,
Contributions to operational energy use during the use stage cardboard and electronics are assumed incinerated with energy
(B6) come from the electricity consumption of the product. The recovery. The residual fractions are landfilled and declared in
annual electricity consumption is calculated by multiplying the C4.
average power input, which is based on a defined load profile,
with the annual running hours. For use stage (B6) European The specific amounts are shown in the scenarios section.
Average electricity grid mix has been used. These values are
declared in the scenarios section. Beyond system boundary (D): According to EN 15804
module D includes the reuse, recovery and/or recycling
The End-of-Life stage (C1-C4) includes all activities from potentials, expressed as net impacts and benefits. Any
when the product reaches the end of its service life and no declared benefits and loads from net flows leaving the product
longer provides any functionality and until all materials and system that have not been allocated as co-products and that
components are processed for reuse/recycling or disposed of. have passed the end-of waste state are included in module D.
According to EN 15804 and the PCR Part A, the end-of-life Contributions to module D comes from waste incineration
stage includes: processes in A5 and C3 as well as material recycling in C3. The
specific fractions and net flows are shown in the scenarios
· C1 deconstruction of the product from the building, including section.
initial on-site sorting of the materials;
Comparability
· C2 transportation of the discarded product to a recycling site
and transportation of waste to final disposal; Basically, a comparison or an evaluation of EPD data is only
possible if all the data sets to be compared were created
· C3 waste processing, collection of waste fractions from the according to EN 15804 and the building context, respectively
deconstruction and waste processing of material flows intended the product-specific characteristics of performance, are taken
for reuse, recycling and energy recovery; into account.
· C4 waste disposal including physical pretreatment and
management of the disposal site. Geographic Representativeness
Land or region, in which the declared product system is
At end of life, the MAGNA3 pump is manually disassembled manufactured, used or handled at the end of the product´s
from the piping system in which it has been installed. The lifespan: Germany
definition of the applied end-of-life scenario in this EPD follows
the requirements in the
Comparability
Basically, a comparison or an evaluation of EPD data is only
PCR Part A, 6.2 regarding complex products, with a
possible if all the data sets to be compared were created
combination of recycling, thermal waste treatment and
according to EN 15804 and the building context, respectively
landfilling. 100 % of the material is considered in the end of life
the product-specific characteristics of performance, are taken
scenario as required by the PCR. An overall collection rate of
into account. Software and databases used: LCA for Experts
90 % has been assumed.
10.7.1.28
Schema 8007
Materials from which energy is recovered in an incineration
Sphera and Ecoinvent databases
process with an R1-value above 0.60 are in this study included
LCA: Scenarios and additional technical information
Characteristic product properties of biogenic carbon
The biogenic carbon content quantifies the amount of biogenic
Transport from the gate to the site (A4)
carbon in a construction product leaving the factory gate, and it
will be separately declared for the product and for any Name Value Unit
accompanying packaging, as required from the PCR Part A. Litres of fuel 0,0332 l/100km
The carbon content of cardboard and paper is assumed to Transport distance 2003 km
46%. Overall, there is an amount of weight-% Carbon in the
Capacity utilisation (including empty runs) 85 %
product leaving the factory gate and has to be considered
Gross density of products transported 383 kg/m3
Information on describing the biogenic Carbon Content at
Wastage during distribution 0,02 %
factory gate
Note: 1 kg of biogenic carbon is equivalent to 44/12 kg of CO2. Installation into the building (A5)
Name ValueUnit Name ValueUnit
kg Packaging waste for incineration (LDPE film) 0,016 kg
Biogenic carbon content in product -
C
Packaging waste for incineration
1,60 kg
Biogenic carbon content in accompanying kg (Paper/Cardboard)
0.74
packaging C
5 Environmental Product Declaration - Grundfos Holding A/S - MAGNA3 50-40/60/80/100/120 F (Stainless Steel) and MAGNA3 32-120 F (Stainless Steel)
An estimated RSL of 10 years can be used to facilitate building
Reuse, recovery and/or recycling potentials (D), relevant
calculations. This is an EU consensus-based estimation,
scenario information
referenced in Appendix 7: Lot 11 – Circulators in Buildings,
Name Value Unit
prepared by AEA Energy & Environment for the European
Commission in the context of the Eco Design Directive. A5, incineration w/energy recov. thermal energy 6,56 MJ
A5, incineration w/energy recov. electric energy 3,52 MJ
Reference service life
C3, steel for recycling (net amounts) -0,354 kg
Name Value Unit
C3, stainless steel for recycling (net amounts) 2,95 kg
Life Span according to the manufacturer 10 a
C3, aluminium for recycling (net amounts) -0,454 kg
Operational energy use (B6) C3, copper for recycling (net amounts) 0,248 kg
Name Value Unit C3, incineration w/energy recov. thermal energy 12,5 MJ
Electricity consumption Group 1 335 kWh/a C3, incineration w/energy recov. electric energy. 6,97 MJ
Electricity consumption Group 2 555 kWh/a
Electricity consumption Group 3 715 kWh/a
Average power input, Group 1 0,067 kW
Average power input, Group 2 0,111 kW
Average power input, Group 3 0,143 kW
Running hours (all groups) 5.000 h/a
End of life (C1-C4)
Name Value Unit
Collected as mixed construction waste 18,937 kg
Transportation distance (C2) 500 km
Aluminium for recycling 2,74 kg
Steel for recycling 1,03 kg
Copper for recycling 0,52 kg
Stainless steel for recycling 9,98 kg
Plastics for incineration w/energy 1,34 kg
Electronics for incineration w/energy 0,81 kg
Landfilling 2,52 kg
6 Environmental Product Declaration - Grundfos Holding A/S - MAGNA3 50-40/60/80/100/120 F (Stainless Steel) and MAGNA3 32-120 F (Stainless Steel)
LCA: Results
Characterization model: EN 15804 - 2012+A2 - 2019, PEF. By Decision no. 20170712-n of the IBU SVR, the modules B3, B4, B5 are
marked as MNR (module not relevant) as default. The LCA results in module B6 are given over a period of one year, according to PCR
Part B. To obtain the results from module B6 over the entire life cycle, the LCA results of module B6 must be multiplied by the
estimated RSL of 10 years. The indicator results for module B6 are declared for Group 1. B6 indicator results for other groups can be
derived by multiplying the B6 indicator results with the following factors:
MAGNA3 50-40 F: 1,00
MAGNA3 50-60 F: 1,64
MAGNA3 50-80 F: 2,13
MAGNA3 50-100 F: 2,75
MAGNA3 50-120 F: 3,4
MAGNA3 32-120 F: 2,27
DESCRIPTION OF THE SYSTEM BOUNDARY (X = INCLUDED IN LCA; MND = MODULE OR INDICATOR NOT DECLARED; MNR
= MODULE NOT RELEVANT)
Benefits and
Construction loads beyond
Product stage Use stage End of life stage
process stage the system
boundaries
la ire ta m w a Ry lp p u s tro p s n a rT g n iru tc a fu n a M e h t m o rf tro p s n a rTe tis e h t o t e ta g y lb m e s s A e s U e c n a n e tn ia M ria p e R tn e m e c a lp e R tn e m h s ib ru fe R y g re n e la n o ita re p Oe s u re ta w la n o ita re p Oe s u n o itc u rts n o c -e Dn o itilo m e d tro p s n a rT g n is s e c o rp e ts a W la s o p s iD -e s u e R-y re v o c e R-g n ilc y c e Rla itn e to p
A1 A2 A3 A4 A5 B1 B2 B3 B4 B5 B6 B7 C1 C2 C3 C4 D
X X X X X X X MNR MNR MNR X X X X X X X
RESULTS OF THE LCA - ENVIRONMENTAL IMPACT according to EN 15804+A2: 1PCS of MAGNA3 50-40/60/80/100/120 F and
MAGNA3 32-120 F
Parameter Unit A1 A2 A3 A4 A5 B1 B2 B6 B7 C1 C2 C3 C4 D
GWP-total kg CO 2 eq 1.05E+02 4.69E+00 1.02E+00 1.57E+00 2.38E+00 0 0 1.09E+02 0 0 6.42E-01 5.73E+00 1.2E-01 -8.59E+00
GWP-fossil kg CO 2 eq 1.05E+02 4.69E+00 3.6E+00 1.58E+00 1.11E-01 0 0 1.08E+02 0 0 6.45E-01 5.72E+00 1.21E-01 -8.57E+00
GWP- -2.62E
biogenic kg CO 2 eq -8.02E-03 -7.13E-03 +00 -2.33E-02 2.27E+00 0 0 9.39E-01 0 0 -9.53E-03 1.3E-02 -1.5E-03 -2.17E-02
GWP-luluc kg CO 2 eq 6.48E-02 6.87E-03 2.9E-02 1.43E-02 7.18E-05 0 0 1.17E-02 0 0 5.99E-03 1.91E-04 1.1E-04 -2.78E-03
kg CFC11
ODP 4.74E-08 3.66E-13 4.06E-09 1.06E-11 2.96E-13 0 0 1.99E-09 0 0 8.41E-14 2.82E-11 2.03E-13 -2.06E-11
eq
AP mol H+ eq 7.67E-01 1.41E-01 1.84E-02 9.49E-03 6.86E-04 0 0 2.31E-01 0 0 3.88E-03 3.88E-03 3.75E-04 -8.31E-02
EP-
kg P eq 1.5E-03 3.58E-06 5.94E-05 5.99E-06 1.15E-07 0 0 4.03E-04 0 0 2.36E-06 7.97E-06 1.4E-05 -1.2E-05
freshwater
EP-marine kg N eq 8.37E-02 3.35E-02 3.59E-03 4.55E-03 2.54E-04 0 0 5.52E-02 0 0 1.89E-03 9.93E-04 8.94E-05 -9.47E-03
EP-terrestrial mol N eq 8.97E-01 3.67E-01 3.61E-02 5.05E-02 3.15E-03 0 0 5.77E-01 0 0 2.1E-02 1.12E-02 9.81E-04 -1.02E-01
kg
POCP NMVOC 2.64E-01 9.46E-02 1.02E-02 8.68E-03 6.59E-04 0 0 1.47E-01 0 0 3.59E-03 2.66E-03 2.82E-04 -3.06E-02
eq
ADPE kg Sb eq 8.49E-03 8.48E-08 6.04E-05 1.81E-06 3.1E-09 0 0 1.67E-05 0 0 4.29E-08 2.36E-07 3.26E-09 -1.14E-03
ADPF MJ 1.47E+03 5.83E+01 5.35E+01 2.17E+01 8.43E-01 0 0 2.27E+03 0 0 8.81E+00 3.28E+01 1.81E+00 -9.99E+01
m3 world
WDP eq 3.63E+01 1.55E-02 1.16E-02 2.71E-02 2.94E-01 0 0 2.41E+01 0 0 7.81E-03 7.44E-01 -1.69E-03 -5.87E-01
deprived
GWP = Global warming potential; ODP = Depletion potential of the stratospheric ozone layer; AP = Acidification potential of land and water; EP =
Eutrophication potential; POCP = Formation potential of tropospheric ozone photochemical oxidants; ADPE = Abiotic depletion potential for non-fossil
resources; ADPF = Abiotic depletion potential for fossil resources; WDP = Water (user) deprivation potential)
RESULTS OF THE LCA - INDICATORS TO DESCRIBE RESOURCE USE according to EN 15804+A2: 1PCS of MAGNA3 50-
40/60/80/100/120 F and MAGNA3 32-120 F
Parameter Unit A1 A2 A3 A4 A5 B1 B2 B6 B7 C1 C2 C3 C4 D
PERE MJ 3.92E+02 9.39E-01 4.74E+01 1.68E+00 1.89E-01 0 0 1.36E+03 0 0 6.41E-01 1.92E+01 1.63E-01 6.2E+00
PERM MJ 0 0 0 0 0 0 0 0 0 0 0 0 0 0
PERT MJ 3.92E+02 9.39E-01 4.74E+01 1.68E+00 1.89E-01 0 0 1.36E+03 0 0 6.41E-01 1.92E+01 1.63E-01 6.2E+00
-9.97E
PENRE MJ 1.48E+03 5.84E+01 5.36E+01 2.17E+01 8.43E-01 0 0 2.27E+03 0 0 8.84E+00 3.28E+01 1.82E+00
+01
PENRM MJ 0 0 0 0 0 0 0 0 0 0 0 0 0 0
-9.97E
PENRT MJ 1.48E+03 5.84E+01 5.36E+01 2.17E+01 8.43E-01 0 0 2.27E+03 0 0 8.84E+00 3.28E+01 1.82E+00
+01
SM kg 1.21E+01 0 2.31E-01 2.46E-03 0 0 0 0 0 0 0 0 0 0
RSF MJ 1.46E-23 0 0 2.91E-27 0 0 0 0 0 0 0 0 0 0
NRSF MJ 1.71E-22 0 0 3.42E-26 0 0 0 0 0 0 0 0 0 0
FW m3 1.07E+00 1.08E-03 1.9E-02 1.94E-03 6.92E-03 0 0 1.1E+00 0 0 7.02E-04 2.49E-02 1.89E-05 2.72E-02
7 Environmental Product Declaration - Grundfos Holding A/S - MAGNA3 50-40/60/80/100/120 F (Stainless Steel) and MAGNA3 32-120 F (Stainless Steel)
PERE = Use of renewable primary energy excluding renewable primary energy resources used as raw materials; PERM = Use of renewable primary
energy resources used as raw materials; PERT = Total use of renewable primary energy resources; PENRE = Use of non-renewable primary energy
excluding non-renewable primary energy resources used as raw materials; PENRM = Use of non-renewable primary energy resources used as raw
materials; PENRT = Total use of non-renewable primary energy resources; SM = Use of secondary material; RSF = Use of renewable secondary fuels;
NRSF = Use of non-renewable secondary fuels; FW = Use of net fresh water
RESULTS OF THE LCA – WASTE CATEGORIES AND OUTPUT FLOWS according to EN 15804+A2:
1PCS of MAGNA3 50-40/60/80/100/120 F and MAGNA3 32-120 F
Parameter Unit A1 A2 A3 A4 A5 B1 B2 B6 B7 C1 C2 C3 C4 D
HWD kg 7.01E-06 1.83E-10 1.21E-04 2.57E-08 2.37E-11 0 0 2.67E-07 0 0 2.74E-11 3.78E-09 1.52E-10 -1.84E-03
NHWD kg 8E+00 5.95E-03 3.62E-01 5.1E-03 7.79E-02 0 0 1.67E+00 0 0 1.35E-03 5.13E-01 2.1E+00 1.99E+00
RWD kg 5.03E-02 7.56E-05 1.64E-03 5.45E-05 4E-05 0 0 3.62E-01 0 0 1.65E-05 5.09E-03 2.13E-05 -1.54E-03
CRU kg ND ND ND ND ND ND ND ND ND ND ND ND ND ND
MFR kg 0 0 0 0 0 0 0 0 0 0 0 1.43E+01 0 0
MER kg ND ND ND ND ND ND ND ND ND ND ND ND ND ND
EEE MJ 0 0 0 0 3.62E+00 0 0 0 0 0 0 6.97E+00 0 0
EET MJ 0 0 0 0 6.56E+00 0 0 0 0 0 0 1.25E+01 0 0
HWD = Hazardous waste disposed; NHWD = Non-hazardous waste disposed; RWD = Radioactive waste disposed; CRU = Components for re-use;
MFR = Materials for recycling; MER = Materials for energy recovery; EEE = Exported electrical energy; EET = Exported thermal energy
RESULTS OF THE LCA – additional impact categories according to EN 15804+A2-optional:
1PCS of MAGNA3 50-40/60/80/100/120 F and MAGNA3 32-120 F
Parameter Unit A1 A2 A3 A4 A5 B1 B2 B6 B7 C1 C2 C3 C4 D
Disease
PM 9.52E-06 2.43E-06 2.7E-07 6.14E-08 3.82E-09 0 0 1.94E-06 0 0 2.46E-08 3.25E-08 3.81E-09 -2.03E-06
incidence
kBq U235
IR 6.64E+00 1.09E-02 2.63E-01 8.02E-03 6.32E-03 0 0 6.02E+01 0 0 2.47E-03 8.47E-01 3.16E-03 -6.8E-02
eq
ETP-fw CTUe 7.6E+02 4.13E+01 1.87E+01 1.53E+01 3.83E-01 0 0 6.32E+02 0 0 6.31E+00 9.43E+00 1.14E+00 -1.24E+01
HTP-c CTUh 1.88E-05 7.67E-10 6.46E-07 4.21E-09 2.12E-11 0 0 3.35E-08 0 0 1.28E-10 5.24E-10 7.32E-11 -4.04E-07
HTP-nc CTUh 1.61E-06 2.63E-08 3.94E-08 1.4E-08 5.93E-10 0 0 5.33E-07 0 0 5.7E-09 1.02E-08 6.25E-09 -4.79E-08
SQP SQP 3.56E+02 4.34E+00 8.73E+01 8.92E+00 2.55E-01 0 0 8.93E+02 0 0 3.68E+00 1.27E+01 1.62E-01 -1.66E+01
PM = Potential incidence of disease due to PM emissions; IR = Potential Human exposure efficiency relative to U235; ETP-fw = Potential comparative
Toxic Unit for ecosystems; HTP-c = Potential comparative Toxic Unit for humans (cancerogenic); HTP-nc = Potential comparative Toxic Unit for humans
(not cancerogenic); SQP = Potential soil quality index
Disclaimer 1 – for the indicator 'Potential Human exposure efficiency relative to U235'. This impact category deals mainly with the
eventual impact of low-dose ionizing radiation on human health of the nuclear fuel cycle. It does not consider effects due to possible
nuclear accidents, occupational exposure or radioactive waste disposal in underground facilities. Potential ionizing radiation from the
soil, from radon and from some construction materials is also not measured by this indicator. Disclaimer 2 – for the indicators 'abiotic
depletion potential for non-fossil resources', 'abiotic depletion potential for fossil resources', 'water (user) deprivation potential,
deprivation-weighted water consumption', 'potential comparative toxic unit for ecosystems', 'potential comparative toxic unit for humans
– cancerogenic', 'Potential comparative toxic unit for humans - not cancerogenic', 'potential soil quality index'. The results of this
environmental impact indicator shall be used with care as the uncertainties on these results are high as there is limited experience with
the indicator.
Disclaimer 3: JRC Technical Reports, Version 2, 2018 Page 6, for the indicator "EP-freshwater". This indicator has been calculated as
'kg P eq' as required in the characterization model EUTREND model, Struijs et al., 2009b, as implemented in ReCiPe; This EPD was
created using a software tool.
References
Standards DIRECTIVE 2014/30/EU OF THE EUROPEAN
Machinery Directive PARLIAMENT AND OF THE COUNCIL of 26 February
DIRECTIVE 2006/42/EC OF THE EUROPEAN 2014 on the harmonization of the laws of the Member
PARLIAMENT AND OF THE COUNCIL of 17 May States relating to electromagnetic compatibility
2006 on machinery Ecodesign Directive
Radio Equipment Directive DIRECTIVE 2009/125/EC OF THE EUROPEAN
DIRECTIVE 2014/53/EU OF THE EUROPEAN PARLIAMENT PARLIAMENT AND OF THE COUNCIL of 21 October
AND OF THE COUNCIL of 16 April 2014 on the harmonization
of the laws of the Member States relating to the making 2009 establishing a framework for the setting of
available on the market of
ecodesign requirements for energy-related products
radio equipment
EC 641/2009
Electromagnetic Compatibility (EMC) Directive
COMMISSION REGULATION (EC) No 641/2009 of 22 July
8 Environmental Product Declaration - Grundfos Holding A/S - MAGNA3 50-40/60/80/100/120 F (Stainless Steel) and MAGNA3 32-120 F (Stainless Steel)
2009 implementing Directive 2005/32/EC of the European and similar apparatus – Part 2: Immunity – Product
Parliament and of the Council with regard to ecodesign
requirements for glandless standalone circulators and family standard (CISPR 14-2:2015)
glandless circulators integrated in
EN 50581:2012
products
EN 50581:2012, Technical documentation for the
EC 622/2012
assessment of electrical and electronic products with
COMMISSION REGULATION (EU) No 622/2012 of 11 July
2012 amending Regulation (EC) No 641/2009 with regard to respect to the restriction of hazardous substances
ecodesign requirements for glandless standalone circulators
and glandless circulators integrated in products EN 60335-1
DIRECTIVE 2011/65/EU EN 60335-1:2012/A11:2014/A13:2017, Household
DIRECTIVE 2011/65/EU OF THE EUROPEAN and similar electrical appliances – Safety – Part 1:General
requirements
PARLIAMENT AND OF THE COUNCIL of 8 June 2011
EN 60335-2-51
on the restriction of the use of certain hazardous
EN 60335-2-51:2003-03 + A1:2008 + A2:2012, Household and
substances in electrical and electronic equipment similar electrical appliances – Safety –Part 2-51: Particular
requirements for stationary circulation pumps for heating and
DIRECTIVE 2015/863/EU service water installations
DIRECTIVE 2015/863/EU of 31 March 2015 amending EN 61000-3-2
Annex II to Directive 2011/65/EU of the European EN 61000-3-2:2014/2019, Electromagnetic compatibility (EMC)
– Part 3-2: Limits – Limits for harmonic current emissions
Parliament and of the Council as regards the list of (equipment input current =16 A per phase)
restricted substances EN 61000-3-3
ETSI EN 301 489-1 EN 61000-3-3:2013-08/ A1:2019, Electromagnetic compatibility
(EMC) – Part 3-3:
ETSI EN 301 489-1 V2.2.0, Electromagnetic Compatibility Limits – Limitation of voltage changes, voltage fluctuations and
(EMC) standard for radio equipment and services; Part 1: flicker in public low voltage supply systems, for equipment with
Common technical requirements
rated current <= 16 A per phase and not subject to conditional
ETSI EN 301 489-17 connection
ETSI EN 301 489-17 V3.2.0, Electromagnetic Compatibility EN 61000-6-2
(EMC) standard for radio equipment and services; Part 17:
Specific conditions for Broadband Data Transmission Systems EN 61000-6-2:2008/2019, Electromagnetic compatibility (EMC)
– Part 6-2: Generic standards –Immunity for industrial
ETSI EN 300 328 V2.1.1 environments
ETSI EN 300 328 V2.1.1, Wideband transmission systems; EN 16297-1
Data transmission equipment operating in the 2,4 GHz ISM
band and using wide band modulation techniques EN 16297-1:2012-10, Pumps – Rotodynamic pumps –
Glandless circulators – Part 1:
EN 809 General requirements and procedures for testing and
calculation of energy efficiency index (EEI)
EN 809:1998-10 + A1:2009, Pumps and pump units for
EN 16297-2
liquids - Common safety requirements
EN 16297-2:2012-10, Pumps – Rotodynamic pumps –
EN 55014-1 Glandless circulators – Part 2: Calculation of energy efficiency
index (EEI) for standalone circulators
EN 55014-1:2017, Electromagnetic compatibility –
Requirements for household appliances, electric tools and EN 16297-3
similar apparatus – Part 1: Emission
EN 16297-3:2012, Pumps – Rotodynamic pumps –Glandless
EN 55014-2 circulators – Part 3: Energy efficiency index (EEI) for circulators
integrated in products
EN 55014-2:2015, Electromagnetic compatibility –
ISO 14001
Requirements for household appliances, electric tools
EN ISO 14001:2015-09, Environmental management systems -
9 Environmental Product Declaration - Grundfos Holding A/S - MAGNA3 50-40/60/80/100/120 F (Stainless Steel) and MAGNA3 32-120 F (Stainless Steel)
Requirements with guidance for use
ECHA candidate list
ISO 14025
Candidate List of substances of very high concern (SVHCs) for
DIN EN /ISO 14025:2011-10, Environmental labels and authorisation, European Chemicals Agency (ECHA), Helsinki,
declarations — Type III environmental declarations — Finland
Principles and procedures
EUTREND model
EN 15804
Struijs et al., 2009b
EN 15804:2012-04+A1 2013, Sustainability of construction AEA Energy & Environment
works — Environmental Product Declarations — Core rules for
the product category of construction products Circulators in Buildings
PCR Part A Ecoinvent
Institut Bauen und Umwelt e.V., Berlin (pub.): Product Category
Rules for Building-Related Products and Services, Product Ecoinvent v3.9.1
Category Rules for Construction Products from the range of
Environmental Product Declarations of Institut Bauen und LCA for Experts
Umwelt (IBU), Part A: Calculation Rules for the Life Cycle
Assessment and Requirements on the Project Report, Version LCA for Experts 10.7.1.28Schema 8007
1.3.
REACH
PCR Part B
Regulation (EC) No 1907/2006 of the European Parliament and
Institut Bauen und Umwelt e.V., Berlin (pub.): Product Category of the Council of 18 December 2006 concerning the
Rules for Building-Related Products and Services, Product Registration, Evaluation, Authorisation and Restriction of
Category Rules for Construction Products from the range of Chemicals (REACH) (Status: 27.06.2018)
Environmental Product Declarations of Institut Bauen und
Umwelt (IBU), Part B: Requirements on the EPD for Pumps for SVR
liquids and liquids with solids, Version 1.0 (2018)
Advisory Board (formerly SVA)
Further references
Decision no.
CPR 20170712-n
REGULATION (EU) No 305/2011 OF THE EUROPEAN AEA Energy & Environment
PARLIAMENT AND OF THE COUNCIL of 9 March 2011 laying ED02287 Circulators in buildings for the European Commission
down harmonised conditions for the marketing of construction
products and repealing Council Directive 89/106/EEC EUTREND model, Struijs et al., 2009b[BSJ1] ,
CML 2001 EUTREND model
Struijs et al 2009b
Impact assessment characterization factors Institute of
Environmental Sciences, Leiden University, Netherlands
10 Environmental Product Declaration - Grundfos Holding A/S - MAGNA3 50-40/60/80/100/120 F (Stainless Steel) and MAGNA3 32-120 F (Stainless Steel)
Publisher
Institut Bauen und Umwelt e.V. +49 (0)30 3087748- 0
Hegelplatz 1 info@ibu-epd.com
10117 Berlin www.ibu-epd.com
Germany
Programme holder
Institut Bauen und Umwelt e.V. +49 (0)30 3087748- 0
Hegelplatz 1 info@ibu-epd.com
10117 Berlin www.ibu-epd.com
Germany
Author of the Life Cycle Assessment
Grundfos Holding A/S +45 87501400
Poul Due Jensens Vej 7 LCA_EPD@grundfos.com
8850 Bjerringbro www.grundfos.com
Denmark
Owner of the Declaration
Grundfos Holding A/S +45 87501400
Poul Due Jensens Vej 7 LCA_EPD@grundfos.com
8850 Bjerringbro www.grundfos.com
Denmark
11 Environmental Product Declaration - Grundfos Holding A/S - MAGNA3 50-40/60/80/100/120 F (Stainless Steel) and MAGNA3 32-120 F (Stainless Steel)
