ENVIRONMENTAL PRODUCT DECLARATION
as per ISO 14025 and EN 15804+A2
Owner of the Declaration SIGA Cover AG
Programme holder Institut Bauen und Umwelt e.V. (IBU)
Publisher Institut Bauen und Umwelt e.V. (IBU)
Declaration number EPD-SIG-20220185-CBA1-EN
Issue date 24.10.2022
Valid to 23.10.2027
Majrex ® 200
SIGA Cover AG
www.ibu-epd.com | https://epd-online.com
Umwelt Produktdeklaration Name des Herstellers – Name des Produkts
General Information
SIGA Cover AG Majrex ® 200
Programme holder Owner of the declaration
IBU – Institut Bauen und Umwelt e.V. SIGA Cover AG
Panoramastr. 1 Rütmattstrasse 7
10178 Berlin 6017 Ruswil
Germany Switzerland
Declaration number Declared product / declared unit
EPD-SIG-20220185-CBA1-EN Majrex ® 200 / 1m²
This declaration is based on the product Scope:
category rules: This document applies to SIGA Majrex 200 (Majpell 5
False ceiling and underlay sheeting, 11.2017 as public annex), a vapour control layer by the SIGA
(PCR checked and approved by the SVR) Cover AG. It is manufactured in Austria. The declared
unit is 1 m2 with a unit weight of 150 g/m2. The LCA
data were based on production data from the year
Issue date
2020.
24.10.2022
The owner of the declaration shall be liable for the
Valid to
underlying information and evidence; the IBU shall not
23.10.2027
be liable with respect to manufacturer information, life
cycle assessment data and evidences.
The EPD was created according to the specifications
of EN 15804+A2. In the following, the standard will be
simplified as EN 15804.
Verification
The standard EN 15804 serves as the core PCR
Independent verification of the declaration and data
according to ISO 14025:2010
Dipl. Ing. Hans Peters internally x externally
(chairman of Institut Bauen und Umwelt e.V.)
Dr. Alexander Röder Vito D'Incognito
(Managing Director Institut Bauen und Umwelt e.V.)) (Independent verifier)
Product
Product description/Product definition after the screed and plaster have been applied or in
SIGA Majrex® is a high-tech vapor control layer with the event of high moisture exposure during use.
integrated Hygrobrid® technology. Thanks to Hygrobrid
®- technology the humidity within the construction is Technical Data
minimized and the moisture transport out of the
construction is maximized
Name Value Unit
For the placing on the market of the product in the Length acc. to EN 1848-2 50 m
European Union/European Free Trade Association Width acc. to EN 1848-2 1.5 m
(EU/EFTA) (with the exception of Switzerland) Straightness acc. to EN 1848-2 passed mm/10m
Regulation (EU) No. 305/2011 (CPR) applies. The Grammage acc. to EN 1849-2 0.15 kg/m2
product needs a declaration of performance taking into Resistance to water penetration
W1 -
consideration EN 13984:2013, Flexible sheets for acc. to EN 1928 (class)
waterproofing - Plastic and rubber vapour control Water vapor diffusion equivalent
layers - Definitions and characteristics and the CE- air layer thickness acc. to EN 5 -15 m
marking. For the application and use the respective 1931
national provisions apply. Resistance to air penetration acc. m3/m2 h
0.02
to EN 12114 50Pa
Application
Maximum tensile force acc. to EN
SIGA Majrex ® can be used in flat roofs, pitched roofs 300 N/50mm
12311-1
as well as wall constructions. The application is
Elongation acc. to EN 12311-1 35 %
possible in wood construction, metal construction as
Tear Resistance (nail) acc. to EN
well as interior wall insulation in solid construction. 150 N/mm
12310-1
Majrex ® also ensures even more safety in the timber
Flexibility at low temperatures acc. -40 °C
construction in the event of high building moisture -
2 Environmental Product Declaration SIGA – Majrex 200 and Majpell 5
to EN 1109 This product contains substances listed in the
candidate list (date: 01.01.2022) exceeding 0.1
percentage by mass: no.
Performance data of the product in accordance with
the declaration of performance with respect to its Reference service life
essential characteristics according to EN 13984. When installed according to the user manual, the
service life of the products is equal to the service life of
Base materials/Ancillary materials the building element, where the product is a part of
(e.g. wall, roof etc.). The Sustainable Building
Composition SIGA Majrex 200 Assessment System BNB specifies the service life of
Name Value Unit the building elements, where the products are used, as
Fleece Polyethylene terephthalate equal to or more than 50 years. A reference service life
25 - 50 %
(PET) according to ISO 15686 is not reported.
Coating Polyester copolymer 25 - 50 %
Coating Polyamide 6 (PA6) 10 - 25 %
Coating Polyethylene copolymer 10 - 25 %
LCA: Calculation rules
Declared Unit Construction stage - Modules A4-A5
The declared unit is 1m2 of Majrex ® 200 with a The construction process stage includes:
grammage of 150 g/m2.  Transport to the construction site (A4)
 Treatment of packaging material (A5)
Declared unit
Name Value Unit
Declared unit 1 m2 End-of-life stage– Modules C1-C4 and D
Grammage 0.15 kg/m2 The end-of-life stage includes
 Manual dismantling (C1)
 Transport to EoL (C2)
 Thermal treatment (C3). No disposal or
System boundary
landfill processes (C4)
Type of EPD according to EN 15804: "cradle to gate
 Reuse, recovery or recycling potential (D) -
with options, modules C1–C4, and module D". The
beyond system boundary includes credits
following modules are declared: A1–A3, C, D and
additional modules: A4 + A5. from thermal treatment (C3) and packaging
treatment (A5)
Production stage - Modules A1-A3
The product stage includes:
 Raw material supply (A1)
Comparability
 Transport to the manufacturer (A2) Basically, a comparison or an evaluation of EPD data
 Manufacturing (A3), including provision of all is only possible if all the data sets to be compared
materials, products and energy, as well as were created according to EN 15804 and the building
context, respectively the product-specific
waste processing up to the end-of-waste
characteristics of performance, are taken into account.
state.
Background database: GaBi content update package
2021.2
LCA: Scenarios and additional technical information
Characteristic product properties building assessment. The values refer to the declared
Information on biogenic Carbon unit of 1 m2 Majrex ® 200 product.
Transport to the building site (A4)
Information on describing the biogenic Carbon Name Value Unit
Content at factory gate Litres of fuel 0.0003 l/100km
Name Value Unit Transport distance 100 km
Biogenic carbon content in Capacity utilisation (including
0 kg C 61 %
product empty runs)
Biogenic carbon content in Gross unit weight of products
0.0107 kg C 0.150 kg/m²
accompanying packaging transported
Installation into the building (A5)
The following technical scenario information is required Name Value Unit
for the declared modules and optional for non-declared Waste packaging (PE foil) to
0.00144 kg
modules. The following technical information is a basis incineration
for the declared modules or can be used for Waste packaging (wood) to
0.00935 kg
developing specific scenarios in the context of a incineration
3 Environmental Product Declaration SIGA – Majrex 200 and Majpell 5
Waste packaging (Cores carton)
0.0181 kg
to incineration
End of life (C1-C4)
For the End-of-Life stage, the product dismantling (C1)
is done manually without environmental burden (load
free).
The transport to End of Life (C2) is calculated with a
distance of 50 km (with 61% utilization).
The Waste processing scenario adopted (C3) is
thermal treatment of the Majrex ® 200 product. Its
incineration results in benefits, beyond the system
boundary, for thermal energy and electricity under
European conditions.
Name Value Unit
Collected separately (Majrex ®
0.15 kg
200)
Energy recovery 0.15 kg
Reuse, recovery and/or recycling potentials (D),
relevant scenario information
Module D includes the credits of the thermal and
electrical energy generated in Modules A5 and C3 due
to the thermal treatment of packaging and product
waste (Majrex ® 200 product).
Avoided burdens have been calculated by the
inversion of residual grid mix and thermal energy from
natural gas, using European datasets.
A waste incineration plant with R1-value > 0.6 is
assumed.
4 Environmental Product Declaration SIGA – Majrex 200 and Majpell 5
LCA: Results
The following tables display the environmental relevant results according to /EN 15804/ for 1 m2 Majrex ® 200.
DESCRIPTION OF THE SYSTEM BOUNDARY (X = INCLUDED IN LCA; ND = MODULE OR INDICATOR NOT
DECLARED; MNR = MODULE NOT RELEVANT)
BENEFITS AND
CONSTRUCTI LOADS
PRODUCT STAGE ON PROCESS USE STAGE END OF LIFE STAGE BEYOND THE
STAGE SYSTEM
BOUNDARIES
5 Environmental Product Declaration SIGA – Majrex 200 and Majpell 5
lairetam
waR
ylppus tropsnarT
gnirutcafunaM
eht
morf
tropsnarT
etis
eht
ot
etag
ylbmessA esU
ecnanetniaM
riapeR
tnemecalpeR tnemhsibrufeR
ygrene
lanoitarepO esu
retaw
lanoitarepO esu
noitcurtsnoc-eD
noitilomed tropsnarT
gnissecorp
etsaW
lasopsiD -esueR -yrevoceR -gnilcyceR laitnetop
A1 A2 A3 A4 A5 B1 B2 B3 B4 B5 B6 B7 C1 C2 C3 C4 D
X X X X X ND ND MNR MNR MNR ND ND X X X X X
RESULTS OF THE LCA - ENVIRONMENTAL IMPACT according to EN 15804+A2: 1 m² Majrex ® 200
Core Indicator Unit A1-A3 A4 A5 C1 C2 C3 C4 D
GWP-total [kg CO2-Eq.] 1.17E+0 1.08E-3 5.04E-2 0.00E+0 9.09E-4 3.75E-1 0.00E+0 -2.45E-1
GWP-fossil [kg CO2-Eq.] 1.21E+0 1.07E-3 5.39E-3 0.00E+0 8.99E-4 3.75E-1 0.00E+0 -2.44E-1
GWP-biogenic [kg CO2-Eq.] -3.56E-2 3.06E-6 4.50E-2 0.00E+0 2.57E-6 2.37E-5 0.00E+0 -1.22E-3
GWP-luluc [kg CO2-Eq.] 4.21E-4 8.80E-6 6.23E-7 0.00E+0 7.38E-6 1.43E-5 0.00E+0 -1.68E-4
ODP [kg CFC11-Eq.] 2.43E-13 1.37E-19 7.49E-18 0.00E+0 1.15E-19 1.15E-16 0.00E+0 -2.78E-15
AP [mol H+-Eq.] 1.43E-3 1.02E-6 9.97E-6 0.00E+0 8.53E-7 4.80E-5 0.00E+0 -3.19E-4
EP-freshwater [kg PO4-Eq.] 2.78E-6 3.19E-9 1.24E-9 0.00E+0 2.68E-9 1.78E-8 0.00E+0 -3.18E-7
EP-marine [kg N-Eq.] 4.93E-4 3.14E-7 3.47E-6 0.00E+0 2.63E-7 1.31E-5 0.00E+0 -9.06E-5
EP-terrestrial [mol N-Eq.] 5.03E-3 3.77E-6 4.58E-5 0.00E+0 3.16E-6 2.18E-4 0.00E+0 -9.71E-4
POCP [kg NMVOC-Eq.] 2.04E-3 8.76E-7 9.28E-6 0.00E+0 7.34E-7 3.77E-5 0.00E+0 -2.54E-4
ADPE [kg Sb-Eq.] 6.51E-7 8.18E-11 1.14E-10 0.00E+0 6.86E-11 1.67E-9 0.00E+0 -4.05E-8
ADPF [MJ] 2.40E+1 1.43E-2 1.24E-2 0.00E+0 1.20E-2 1.46E-1 0.00E+0 -4.23E+0
[m³ world-Eq
WDP 3.93E-2 9.34E-6 5.33E-3 0.00E+0 7.83E-6 3.90E-2 0.00E+0 -1.87E-2
deprived]
GWP = Global warming potential; ODP = Depletion potential of the stratospheric ozone layer; AP = Acidification potential of land and water; EP =
Caption Eutrophication potential; POCP = Formation potential of tropospheric ozone photochemical oxidants; ADPE = Abiotic depletion potential for non-
fossil resources; ADPF = Abiotic depletion potential for fossil resources; WDP = Water (user) deprivation potential
RESULTS OF THE LCA - INDICATORS TO DESCRIBE RESOURCE USE according to EN 15804+A2: 1 m²
Majrex ® 200
Indicator Unit A1-A3 A4 A5 C1 C2 C3 C4 D
PERE [MJ] 1.32E+0 7.99E-4 4.38E-1 0.00E+0 6.70E-4 3.17E-2 0.00E+0 -9.56E-1
PERM [MJ] 4.35E-1 0.00E+0 -4.35E-1 0.00E+0 0.00E+0 0.00E+0 0.00E+0 0.00E+0
PERT [MJ] 1.75E+0 7.99E-4 2.37E-3 0.00E+0 6.70E-4 3.17E-2 0.00E+0 -9.56E-1
PENRE [MJ] 1.94E+1 1.43E-2 7.86E-2 0.00E+0 1.20E-2 4.68E+0 0.00E+0 -4.23E+0
PENRM [MJ] 4.60E+0 0.00E+0 -6.62E-2 0.00E+0 0.00E+0 -4.53E+0 0.00E+0 0.00E+0
PENRT [MJ] 2.40E+1 1.43E-2 1.24E-2 0.00E+0 1.20E-2 1.46E-1 0.00E+0 -4.23E+0
SM [kg] 0.00E+0 0.00E+0 0.00E+0 0.00E+0 0.00E+0 0.00E+0 0.00E+0 0.00E+0
RSF [MJ] 0.00E+0 0.00E+0 0.00E+0 0.00E+0 0.00E+0 0.00E+0 0.00E+0 0.00E+0
NRSF [MJ] 0.00E+0 0.00E+0 0.00E+0 0.00E+0 0.00E+0 0.00E+0 0.00E+0 0.00E+0
FW [m³] 4.68E-3 9.14E-7 1.26E-4 0.00E+0 7.67E-7 9.25E-4 0.00E+0 -9.34E-4
PERE = Use of renewable primary energy excluding renewable primary energy resources used as raw materials; PERM = Use of
renewable primary energy resources used as raw materials; PERT = Total use of renewable primary energy resources; PENRE = Use of
non-renewable primary energy excluding non-renewable primary energy resources used as raw materials; PENRM = Use of non-
Caption
renewable primary energy resources used as raw materials; PENRT = Total use of non-renewable primary energy resources; SM = Use
of secondary material; RSF = Use of renewable secondary fuels; NRSF = Use of non-renewable secondary fuels; FW = Use of net fresh
water
RESULTS OF THE LCA – WASTE CATEGORIES AND OUTPUT FLOWS according to EN 15804+A2:
1 m² Majrex ® 200
Indicator Unit A1-A3 A4 A5 C1 C2 C3 C4 D
HWD [kg] 8.84E-9 7.22E-13 2.28E-12 0.00E+0 6.05E-13 2.62E-11 0.00E+0 -9.51E-10
NHWD [kg] 1.37E-2 2.13E-6 9.43E-4 0.00E+0 1.78E-6 3.62E-2 0.00E+0 -1.99E-3
RWD [kg] 1.83E-4 1.73E-8 6.50E-7 0.00E+0 1.45E-8 5.70E-6 0.00E+0 -3.08E-4
CRU [kg] 0.00E+0 0.00E+0 0.00E+0 0.00E+0 0.00E+0 0.00E+0 0.00E+0 0.00E+0
MFR [kg] 0.00E+0 0.00E+0 0.00E+0 0.00E+0 0.00E+0 0.00E+0 0.00E+0 0.00E+0
MER [kg] 0.00E+0 0.00E+0 0.00E+0 0.00E+0 0.00E+0 0.00E+0 0.00E+0 0.00E+0
EEE [MJ] 1.46E-1 0.00E+0 7.28E-2 0.00E+0 0.00E+0 8.30E-1 0.00E+0 0.00E+0
EET [MJ] 2.76E-1 0.00E+0 1.31E-1 0.00E+0 0.00E+0 1.50E+0 0.00E+0 0.00E+0
HWD = Hazardous waste disposed; NHWD = Non-hazardous waste disposed; RWD = Radioactive waste disposed; CRU = Components
Caption for re-use; MFR = Materials for recycling; MER = Materials for energy recovery; EEE = Exported electrical energy; EET = Exported
thermal energy
RESULTS OF THE LCA – additional impact categories according to EN 15804+A2-optional:
1 m² Majrex ® 200
Indicator Unit A1-A3 A4 A5 C1 C2 C3 C4 D
[Disease
PM 1.24E-8 6.21E-12 5.40E-11 0.00E+0 5.20E-12 6.78E-10 0.00E+0 -2.74E-9
Incidence]
[kBq U235-
IRP 2.16E-2 2.48E-6 1.02E-4 0.00E+0 2.08E-6 7.47E-4 0.00E+0 -5.05E-2
Eq.]
ETP-fw [CTUe] 9.87E+0 1.03E-2 5.67E-3 0.00E+0 8.67E-3 1.05E-1 0.00E+0 -8.86E-1
HTP-c [CTUh] 4.91E-10 2.09E-13 3.42E-13 0.00E+0 1.75E-13 5.69E-12 0.00E+0 -4.03E-11
HTP-nc [CTUh] 3.88E-8 1.08E-11 1.39E-11 0.00E+0 9.04E-12 6.12E-10 0.00E+0 -1.59E-9
SQP [-] 4.28E+0 4.91E-3 3.29E-3 0.00E+0 4.12E-3 3.56E-2 0.00E+0 -6.54E-1
PM = Potential incidence of disease due to PM emissions; IR = Potential Human exposure efficiency relative to U235; ETP-fw = Potential
Caption comparative Toxic Unit for ecosystems; HTP-c = Potential comparative Toxic Unit for humans (cancerogenic); HTP-nc = Potential
comparative Toxic Unit for humans (not cancerogenic); SQP = Potential soil quality index
Disclaimer 1 – for the indicator “Potential Human exposure efficiency relative to U235”.
This impact category deals mainly with the eventual impact of low dose ionizing
radiation on human health of the nuclear fuel cycle. It does not consider effects due to possible
nuclear accidents, occupational exposure nor due to radioactive waste disposal in underground
facilities. Potential ionizing radiation from the soil, from radon and from some construction materials is also not
measured by this indicator.
Disclaimer 2 – for the indicators “abiotic depletion potential for non-fossil resources”, “abiotic depletion potential
for fossil resources”, “water (user) deprivation potential, deprivation-weighted water consumption”, “potential
comparative toxic unit for ecosystems”, “potential comparative toxic unit for humans – cancerogenic”, “Potential
comparative toxic unit for humans - not cancerogenic”, “potential soil quality index”.
The results of this environmental impact indicator shall be used with care as the
uncertainties on these results are high or as there is limited experienced with the indicator.
References
Product related standards resistance to tearing (nail shank); German version
EN 12310-1:1999
Assessment System for Sustainable Building
2014-09
assessment_system_bnb.pdf (bnb- EN 12311-1:1999
nachhaltigesbauen.de) Flexible sheets for waterproofing - Part 1: Bitumen
sheets for roof waterproofing; Determination of tensile
EN 1109:2013 properties; German version EN 12311-1:1999
Flexible sheets for waterproofing - Bitumen sheets for
roof waterproofing - Determination of flexibility at low EN 13984:2013
temperature; German version EN 1109:2013 Flexible sheets for waterproofing - Plastic and rubber
vapour control layers - Definitions and characteristics;
EN 1848-2:2001 German version EN 13984:2013
Flexible sheets for waterproofing - Determination of
length, width, straightness and flatness - Part 2: Plastic ISO 15686-1:2011
and rubber sheets for roof waterproofing; German Buildings and constructed assets - Service life
version EN 1848-2:2001 planning - Part 1: General principles and framework
EN 1928:2000 regulation (EU) No 305/2011
Flexible sheets for waterproofing - Bitumen, plastic and EUR-Lex - 32011R0305 - EN - EUR-Lex (europa.eu)
rubber sheets for roof waterproofing - Determination of
watertightness; German version EN 1928:2000 the candidate list
List of substances of very high concern for
EN 1931:2001 authorisation - ECHA (europa.eu)
Flexible sheets for waterproofing - Bitumen, plastic and
rubber sheets for roof waterproofing - Determination of
water vapour transmission properties; German version Standards
EN 1931:2000
EN 15804
EN 12114:2000 EN 15804:2019+A2, Sustainability of construction
Thermal performances of buildings - Air permeability of works — Environmental Product Declarations — Core
building components and building elements - rules for the product category of construction products.
Laboratory test method; German version
EN 12114:2000 ISO 14025
DIN EN ISO 14025:2011-10, Environmental labels and
EN 12310-1:1999 declarations — Type III environmental declarations —
Flexible sheets for waterproofing - Part 1: Bitumen Principles and procedures.
sheets for roof waterproofing; determination of
6 Environmental Product Declaration SIGA – Majrex 200 and Majpell 5
Institut Bauen und Umwelt e.V.: General Programme
Instructions for the Preparation of EPDs at the Institut
Bauen und Umwelt e.V. Version 2.0., Berlin: Institut
Bauen und Umwelt e.V., 2021
Further References
PCR Part A
CPR PCR - Part A: Calculation rules for the Life Cycle
Regulation No. 305/2011: Construction Products Assessment and Requirements on the Background
Regulation of the European Parliament and of the Report, version 2.1, Institut Bauen und Umwelt e.V.,
European Council, 2011. 2021, www.bau-umwelt.com
GaBi ts PCR Part B
GaBi ts dataset documentation for the software-system PCR – Part B: Requirements on the EPD for False
and databases, LBP, University of Stuttgart and ceiling and underlay sheeting, version 1.6, 2017,
thinkstep, Leinfelden-Echterdingen, 2021 Institut Bauen und Umwelt e.V., www.bau-umwelt.com
(https://www.gabi-software.com/support/gabi)
IBU 2021
7 Environmental Product Declaration SIGA – Majrex 200 and Majpell 5
Publisher
Institut Bauen und Umwelt e.V. Tel +49 (0)30 3087748- 0
Panoramastr. 1 Fax +49 (0)30 3087748- 29
10178 Berlin Mail info@ibu-epd.com
Germany Web www.ibu-epd.com
Programme holder
Institut Bauen und Umwelt e.V. Tel +49 (0)30 - 3087748- 0
Panoramastr 1 Fax +49 (0)30 – 3087748 - 29
10178 Berlin Mail info@ibu-epd.com
Germany Web www.ibu-epd.com
Author of the Life Cycle
Assessment Tel +49 711 341817-0
Sphera Solutions GmbH Fax +49 711 341817-25
Hauptstraße 111- 113 Mail info@sphera.com
70771 Leinfelden-Echterdingen Web www.sphera.com
Germany
Owner of the Declaration
SIGA Cover AG Tel 0041 41 499 69 69
Rüttmatstrasse 7 Fax 0041 41 496 62 63
6017 Ruswil Mail technik@siga.swiss
Switzerland Web www.siga.swiss
