Environmental product declaration
in accordance with ISO 14025 and EN 15804+A2
Marble Block Stone from Norwegian Rose Quarry - China
Owner of the declaration: Program operator:
Norwegian Rose AS The Norwegian EPD Foundation
Product: Declaration number:
Marble Block Stone from Norwegian Rose Quarry - China
Registration number:
Declared unit:
1 tonne Issue date:
This declaration is based on Product Category Rules: Valid to:
CEN Standard EN 15804:2012+A2:2019 serves as core
EPD software:
PCR
The Norwegian EPD Foundation LCAno EPD generator ID: 465481
NPCR 018:2022 Part B for natural stone products,
aggregates and fillers
1 / 11
General information
Product Owner of the declaration:
Marble Block Stone from Norwegian Rose Quarry - China Norwegian Rose AS
Contact person: Susan Moser
Phone: +47 7564 3207
e-mail: info@fauskemarble.com
Program operator: Manufacturer:
The Norwegian EPD Foundation Norwegian Rose AS
Post Box 5250 Majorstuen, 0303 Oslo, Norway
Phone: +47 977 22 020
web: www.epd-norge.no
Declaration number: Place of production:
Norwegian Rose AS
Løvgavlveien 16
8218 Fauske, Norway
This declaration is based on Product Category Rules: Management system:
CEN Standard EN 15804:2012+A2:2019 serves as core PCR
NPCR 018:2022 Part B for natural stone products, aggregates and
fillers
Statement of liability: Organisation no:
The owner of the declaration shall be liable for the underlying 982 422 639
information and evidence. EPD Norway shall not be liable with respect
to manufacturer information, life cycle assessment data and
evidences.​
Declared unit: Issue date:
1 tonne Marble Block Stone from Norwegian Rose Quarry - China
Declared unit with option: Valid to:
A1,A2,A3,A4,C1,C2,C3,C4,D
Year of study:
2023
Functional unit: Comparability:
Not applicable. EPD of construction products may not be comparable if they not
comply with EN 15804 and seen in a building context.
General information on verification of EPD from EPD tools: Development and verification of EPD:
Independent verification of data, other environmental information The declaration is created using EPD tool lca.tools ver EPD2022.03,
and the declaration according to ISO 14025:2010, § 8.1.3 and § 8.1.4. developed by LCA.no. The EPD tool is integrated in the company's
Verification of each EPD is made according to EPD-Norway’s management system, and has been approved by EPD Norway.
guidelines for verification and approval requiring that tools are i)
integrated into the company's environmental management system, ii) Developer of EPD: Pedro Ferreira
the procedures for use of the EPD tool are approved by EPD-Norway,
Reviewer of company-specific input data and EPD:​ Børge Heggen
and iii) the process is reviewed annually by an independent third
Johansen, Energiråd AS
party verifier. See Appendix G of EPD-Norway's General Programme
Instructions for further information on EPD tools
Verification of EPD tool: Approved:
Independent third party verification of the EPD tool, background data
and test-EPD in accordance with EPDNorway's procedures and
guidelines for verification and approval of EPD tools.
Håkon Hauan, CEO EPD-Norge
Third party verifier:
Martin Erlandsson, IVL Swedish Res. Inst
(no signature required)
2 / 11
Product
Product description:
Marble block stone from Fauske is quarried north of the Arctic Circle and characterized by its distinctive patterns and a range of shades and colors.
These versatile blocks can be used as walling stone, exterior wall cladding, interior design, high-traffic flooring, and sculptural artistic work, to name
a few.
Product specification
The petrographic classification of the stone is Calcitic-Dolomitic marble. The marble with its significant Dolomite content is typically more durable
and better suited for high-traffic areas or exterior applications where durability is essential, making the product known for versatile usage. The
stone block comes as squared or shapeless (labeled as Mosaic). The marble comes in three dominating colors:
1. Norwegian Rose, world-renowned pink marble.
2. Hermelin (Antique Fonce), classic blue-grey marble in a dark and light version.
3. Antique Verdatre, exclusive mint green-white marble.
Materials Value Unit
Stone 1000 kg
Technical data:
Mineralogy: Calcite (65%), dolomite (30%), various auxiliary minerals (5%)
The product meets the requirements set by the general reference rules UNI EN 1469/2015 and the chemical and physical properties correspond
to the values specified by the relevant UNI.
Reference standards: EN 1936, 12373, 13755, 1926, 12371.
Physical properties Value Unit
Flexural strength-average value 12.3 MPa
Real density and apparent density and total and open porosity 2760 kg/m³
Water absorption at atmospheric pressure 0.1 %
Uniaxial compressive strength 98 MPa
Frost resistance after 56 cycles -3.6 %
Market:
China.
Reference service life, product
Depending on the application.
Reference service life, building or construction works
The lifespan of buildings is often assumed to be 60 years.
LCA: Calculation rules
Declared unit:
1 tonne Marble Block Stone from Norwegian Rose Quarry - China
Cut-off criteria:
All major raw materials and all the essential energy is included. The production processes for raw materials and energy flows with very small
amounts (less than 1%) are not included. These cut-off criteria do not​ apply for hazardous materials and substances.
Allocation:
The allocation is made in accordance with the provisions of EN 15804. Incoming energy and water and waste production in-house is allocated
equally among all products through mass allocation. Effects of primary production of recycled materials is allocated to the main product in which
the material was used. The recycling process and transportation of the material is allocated to this analysis.
Data quality:
Specific data for the product composition are provided by the manufacturer. The data represent the production of the declared product and were
collected for EPD development in the year of study. Background data is based on EPDs according to EN 15804 and different LCA databases. The
data quality of the raw materials in A1 is presented in the table below.
3 / 11
System boundaries (X=included, MND=module not declared, MNR=module not relevant)
Construction Beyond the system
Product stage Use stage End of life stage
installation stage boundaries
A1 A2 A3 A4 A5 B1 B2 B3 B4 B5 B6 B7 C1 C2 C3 C4 D
X X X X MND MND MND MND MND MND MND MND X X X X X
System boundary:
Modules A1-A4 are included in the document. A1-A3 encompass the extraction of raw materials, transportation of those materials, and the
manufacturing of shapeless and regular blocks. Both products share the processes of marble extraction from the quarry, internal transportation,
cutting, and splitting. Regular blocks also undergo cutting, final inspection, and storage before being transported to markets in module A4. The
blocks are exported to European countries, where natural stone factories handle further processing into various marble products.
Additional technical information:
Not applicable.
waR slairetam tropsnarT gnirutcafunaM tropsnarT ylbmessA e​sU ecnanetniaM riapeR tnemecalpeR tnemhsibrufeR lanoitarepO ygrene esu lanoitarepO esu retaw -eD noitcurtsnoc noitilomed tropsnarT etsaW gnissecorp lasopsiD -yrevoceR-esueR laitnetop-gnilcyceR
4 / 11
LCA: Scenarios and additional technical information
The following information describe the scenarios in the different modules of the EPD.
The square and shapeless blocks are distributed to clients in China. The method of transport is a combination of truck, rail and container ship.
Modules C and D present average values for the end-of-life stages of natural stone products, based on Norwegian statistics. 50 km in module C2
is used as the industry average.
Capacity utilisation Value
Transport from production place to user (A4) Distance (km) Fuel/Energy Consumption Unit
(incl. return) % (Liter/tonne)
Ship, freight 150 000 DWT (km) 65,0 % 27550 0,003 l/tkm 82,65
Train, unspecified (km) - Global 0,0 % 1221 0,009 l/tkm 10,99
Truck, over 32 tonnes, EURO 6 (km) 53,3 % 116 0,023 l/tkm 2,66
De-construction demolition (C1) Unit Value
Demolition of stone materials (kg) kg/DU 1000,00
Capacity utilisation Value
Transport to waste processing (C2) Distance (km) Fuel/Energy Consumption Unit
(incl. return) % (Liter/tonne)
Truck, 16-32 tonnes, EURO 6 (km) 36,7 % 50 0,043 l/tkm 2,15
Waste processing (C3) Unit Value
Waste treatment of stone products after
kg/DU 700,00
demolition (kg)
Disposal (C4) Unit Value
Waste, stone, for landfill (kg) kg/DU 300,00
Benefits and loads beyond the system
Unit Value
boundaries (D)
Substitution of stone materials (kg) kg/DU 700,00
5 / 11
LCA: Results
The LCA results are presented below for the declared unit defined on page 2 of the EPD document.
Environmental impact
Shapeless Squared
Indicator Unit A4 C1 C2 C3 C4 D
Blocks Blocks
GWP-total kg CO2 -eq 2,93E+01 2,08E+01 3,27E+02 4,00E+00 8,17E+00 5,04E-01 1,29E+00 -1,64E+00
GWP-fossil kg CO2 -eq 2,92E+01 2,07E+01 3,27E+02 4,00E+00 8,17E+00 4,97E-01 1,28E+00 -1,60E+00
GWP-biogenic kg CO2 -eq 7,37E-02 7,39E-02 1,86E-01 7,50E-04 3,38E-03 4,29E-03 1,09E-03 -3,20E-02
GWP-luluc kg CO2 -eq 4,01E-03 4,09E-03 2,61E-01 3,15E-04 2,91E-03 6,88E-04 2,52E-04 -1,08E-03
ODP kg CFC11 -eq 6,16E-06 4,30E-06 6,61E-05 8,64E-07 1,85E-06 9,80E-08 6,26E-07 -2,92E-07
AP mol H+ -eq 3,00E-01 2,11E-01 8,99E+00 4,19E-02 2,35E-02 4,02E-03 1,25E-02 -1,44E-02
EP-FreshWater kg P -eq 1,49E-04 1,30E-04 2,76E-03 1,46E-05 6,53E-05 3,14E-05 9,59E-06 -4,26E-05
EP-Marine kg N -eq 1,31E-01 9,15E-02 2,28E+00 1,85E-02 4,64E-03 1,18E-03 4,70E-03 -5,00E-03
EP-Terrestial mol N -eq 1,44E+00 1,00E+00 2,54E+01 2,00E-01 5,19E-02 1,36E-02 5,18E-02 -5,88E-02
POCP kg NMVOC -eq 3,96E-01 2,76E-01 6,61E+00 5,57E-02 1,99E-02 3,64E-03 1,48E-02 -1,55E-02
ADP-minerals&metals1 kg Sb-eq 7,58E-05 7,64E-05 2,56E-03 6,14E-06 2,26E-04 6,31E-06 1,14E-05 -1,42E-04
ADP-fossil1 MJ 3,99E+02 2,82E+02 4,23E+03 5,51E+01 1,23E+02 1,54E+01 4,15E+01 -2,71E+01
WDP1 m3 9,19E+02 1,35E+03 1,74E+03 1,17E+01 1,19E+02 1,70E+03 8,73E+01 -1,27E+03
GWP-total = Global Warming Potential total; GWP-fossil = Global Warming Potential fossil fuels; GWP-biogenic = Global Warming Potential biogenic; GWP-luluc =
Global Warming Potential land use and land use change; ODP = Depletion potential of the stratospheric ozone layer; AP = Acidification potential, Accumulated
Exceedance; EP-freshwater = Eutrophication potential, fraction of nutrients reaching freshwater end compartment: EP-marine = Eutrophication potential, fraction of
nutrients reaching marine end compartment; EP-terrestrial = Eutrophication potential, Accumulated Exceedance; POCP = Formation potential of tropospheric ozone;
ADP-minerals&metals = Abiotic depletion potential for non-fossil resources; ADP-fossil = Abiotic depletion for fossil resources potential; WDP = Water (user)
deprivation potential, deprivation-weighted water consumption
"Reading example: 9,0 E-03 = 9,0*10-3 = 0,009"
*INA Indicator Not Assessed
1. The results of this environmental impact indicator shall be used with care as the uncertainties on these results are high or as there is limited experienced with the
indicator
Remarks to environmental impacts
6 / 11
Additional environmental impact indicators
Shapeless Squared
Indicator Unit A4 C1 C2 C3 C4 D
Blocks Blocks
PM Disease incidence 7,86E-06 5,47E-06 5,81E-06 5,07E-06 5,00E-07 6,44E-08 2,67E-07 -3,07E-07
IRP2 kgBq U235 -eq 1,78E+00 1,32E+00 1,84E+01 2,40E-01 5,40E-01 2,59E-01 1,80E-01 -2,49E-01
ETP-fw1 CTUe 2,39E+02 1,86E+02 2,94E+03 3,01E+01 9,15E+01 1,09E+01 2,05E+01 -2,79E+01
HTP-c1 CTUh 1,01E-08 8,10E-09 0,00E+00 1,00E-09 0,00E+00 7,00E-10 6,00E-10 -1,40E-09
HTP-nc1 CTUh 2,38E-07 1,90E-07 1,34E-06 2,80E-08 1,00E-07 9,80E-09 1,20E-08 -3,43E-08
SQP1 dimensionless 5,34E+01 3,95E+01 1,12E+03 6,69E+00 8,64E+01 8,73E+00 1,51E+02 6,15E+01
PM = Particulate Matter emissions; IRP = Ionizing radiation – human health; ETP-fw = Eco toxicity – freshwater; HTP-c = Human toxicity – cancer effects; HTP-nc =
Human toxicity – non cancer effects; SQP = Potential Soil Quality Index (dimensionless)
"Reading example: 9,0 E-03 = 9,0*10-3 = 0,009"
*INA Indicator Not Assessed
1. The results of this environmental impact indicator shall be used with care as the uncertainties on these results are high or as there is limited experienced with the
indicator
2. This impact category deals mainly with the eventual impact of low dose ionizing radiation on human health of the nuclear fuel cycle. It does not consider effects due
to possible nuclear accidents, occupational exposure nor due to radioactive waste disposal in underground facilities. Potential ionizing radiation from the soil, from
radon and from some construction materials is also not measured by this indicator.
7 / 11
Resource use
Shapeless Squared
Indicator Unit A4 C1 C2 C3 C4 D
Blocks Blocks
PERE MJ 5,84E+01 9,18E+01 6,89E+01 3,00E-01 1,77E+00 7,95E+00 6,38E-01 -6,35E+00
PERM MJ 0,00E+00 0,00E+00 0,00E+00 0,00E+00 0,00E+00 0,00E+00 0,00E+00 0,00E+00
PERT MJ 5,84E+01 9,18E+01 6,89E+01 3,00E-01 1,77E+00 7,95E+00 6,38E-01 -6,35E+00
PENRE MJ 3,99E+02 2,82E+02 4,23E+03 5,51E+01 1,23E+02 1,54E+01 4,15E+01 -2,86E+01
PENRM MJ 0,00E+00 0,00E+00 0,00E+00 0,00E+00 0,00E+00 0,00E+00 0,00E+00 0,00E+00
PENRT MJ 3,99E+02 2,82E+02 4,23E+03 5,51E+01 1,23E+02 1,54E+01 4,15E+01 -2,86E+01
SM kg 0,00E+00 0,00E+00 0,00E+00 0,00E+00 0,00E+00 0,00E+00 0,00E+00 0,00E+00
RSF MJ 1,49E-01 1,57E-01 1,29E+00 0,00E+00 6,32E-02 0,00E+00 1,32E-02 -1,30E-01
NRSF MJ 9,25E-01 7,55E-01 7,82E+00 0,00E+00 2,26E-01 0,00E+00 3,79E-02 -1,33E-01
FW m3 1,28E+00 1,48E+00 4,93E-01 2,83E-03 1,32E-02 2,64E-02 4,94E-02 -9,96E-01
PERE = Use of renewable primary energy excluding renewable primary energy resources used as raw materials; PERM = Use of renewable primary energy resources used
as raw materials; PERT = Total use of renewable primary energy resources; PENRE = Use of non renewable primary energy excluding non-renewable primary energy
resources used as raw materials; PENRM = Use of non renewable primary energy resources used as raw materials; PENRT = Total use of non renewable primary energy
resources; SM = Use of secondary materials; RSF = Use of renewable secondary fuels; NRSF = Use of non-renewable secondary fuels; FW = Net use of fresh water
"Reading example: 9,0 E-03 = 9,0*10-3 = 0,009"
*INA Indicator Not Assessed
8 / 11
End of life - Waste
Shapeless Squared
Indicator Unit A4 C1 C2 C3 C4 D
Blocks Blocks
HWD kg 1,26E-01 1,18E-01 3,46E-01 1,62E-03 6,37E-03 1,54E-03 0,00E+00 -6,54E-03
NHWD kg 2,58E+00 2,54E+00 3,27E+01 6,52E-02 6,01E+00 4,87E-02 3,00E+02 -1,98E-01
RWD kg 2,77E-03 1,97E-03 2,84E-02 3,82E-04 8,41E-04 1,63E-04 0,00E+00 -2,15E-04
HWD = Hazardous waste disposed; NHWD = Non-hazardous waste disposed; RWD = Radioactive waste disposed
"Reading example: 9,0 E-03 = 9,0*10-3 = 0,009"
*INA Indicator Not Assessed
End of life - Output flow
Shapeless Squared
Indicator Unit A4 C1 C2 C3 C4 D
Blocks Blocks
CRU kg 0,00E+00 0,00E+00 0,00E+00 0,00E+00 0,00E+00 0,00E+00 0,00E+00 0,00E+00
MFR kg 1,62E+00 1,53E+00 0,00E+00 0,00E+00 0,00E+00 7,00E+02 0,00E+00 0,00E+00
MER kg 5,04E-01 4,74E-01 0,00E+00 0,00E+00 0,00E+00 0,00E+00 0,00E+00 0,00E+00
EEE MJ 2,99E-01 2,82E-01 0,00E+00 0,00E+00 0,00E+00 0,00E+00 0,00E+00 0,00E+00
EET MJ 4,53E+00 4,26E+00 0,00E+00 0,00E+00 0,00E+00 0,00E+00 0,00E+00 0,00E+00
CRU = Components for re-use; MFR = Materials for recycling; MER = Materials for energy recovery; EEE = Exported energy electrical; EET = Exported energy thermal
"Reading example: 9,0 E-03 = 9,0*10-3 = 0,009"
*INA Indicator Not Assessed
Biogenic Carbon Content
Indicator Unit At the factory gate
Biogenic carbon content in product kg C 0,00E+00
Biogenic carbon content in accompanying packaging kg C 0,00E+00
Note: 1 kg biogenic carbon is equivalent to 44/12 kg CO2
9 / 11
Additional requirements
Greenhouse gas emissions from the use of electricity in the manufacturing phase
National production mix from import, low voltage (production of transmission lines, in addition to direct emissions and losses in grid) of applied
electricity for the manufacturing process (A3).
Dangerous substances
The product contains no substances given by the REACH Candidate list.
Indoor environment
Additional Environmental Information
Additional environmental impact indicators required in NPCR Part A for construction products
Shapeless Squared
Indicator Unit A4 C1 C2 C3 C4 D
Blocks Blocks
GWPIOBC kg CO2 -eq 2,92E+01 2,07E+01 4,62E+02 4,00E+00 8,17E+00 4,98E-01 1,29E+00 -1,71E+00
GWP-IOBC: Global warming potential calculated according to the principle of instantaneous oxidation. In order to increase the transparency of biogenic carbon​
contribution to climate impact, the indicator GWP-IOBC is required as it declares climate impacts calculated according to the principle of instantaneous oxidation.​
GWP-IOBC is also referred to as GWP-GHG in context to Swedish public procurement legislation.
10 / 11
Bibliography
ISO 14025:2010 Environmental labels and declarations - Type III environmental declarations - Principles and procedures.
ISO 14044:2006 Environmental management - Life cycle assessment - Requirements and guidelines.
EN 15804:2012+A2:2019 Environmental product declaration - Core rules for the product category of construction products.
ISO 21930:2017 Sustainability in buildings and civil engineering works - Core rules for environmental product declarations of construction
products.
ecoinvent v3, Allocation, cut-off by classification, Swiss Centre of Life Cycle Inventories.
Iversen et al., (2021) eEPD v2021.09 Background information for EPD generator tool system verification, LCA.no Report number: 07.21
Vold, M., and Iversen, O. M. K. (2022) EPD generator for for NPCR 018 Part B for natural stone products, aggregates and fillers
Background information for EPD generator application and LCA data, LCA.no report number: 09.22.
NPCR Part A: Construction products and services. Ver. 2.0, 24.03.2021 EPD Norway.
NPCR 018 Part B for natural stone products, aggregates and fillers, Ver. 1.1, 20.01.2022, EPD Norway.
Program operator and publisher Phone: +47 977 22 020
The Norwegian EPD Foundation e-mail: post@epd-norge.no
Post Box 5250 Majorstuen, 0303 Oslo, Norway web: www.epd-norge.no
Owner of the declaration: Phone: +47 7564 3207
Norwegian Rose AS e-mail: info@fauskemarble.com
Løvgavlveien 16, 8218 Fauske web: www.fauskemarble.com
Author of the Life Cycle Assessment Phone: +47 916 50 916
LCA.no AS e-mail: post@lca.no
Dokka 6A, 1671 web: www.lca.no
Developer of EPD generator Phone: +47 916 50 916
LCA.no AS e-mail: post@lca.no
Dokka 6B,1671 Kråkerøy web: www.lca.no
ECO Platform web: www.eco-platform.org
ECO Portal web: ECO Portal
11 / 11
