ENVIRONMENTAL PRODUCT DECLARATION
as per ISO 14025 and EN 15804+A2
Owner of the Declaration Hilti Aktiengesellschaft
Publisher Institut Bauen und Umwelt e.V. (IBU)
Programme holder Institut Bauen und Umwelt e.V. (IBU)
Declaration number EPD-HIL-20230439-IBA1-EN
Issue date 18/12/2023
Valid to 17/12/2028
MFT FOX H & MFT S2S
Hilti AG
www.ibu-epd.com | https://epd-online.com
General Information
Hilti AG MFT FOX H & MFT S2S
Programme holder Owner of the declaration
IBU – Institut Bauen und Umwelt e.V. Hilti Aktiengesellschaft
Hegelplatz 1 Feldkircher Strasse 100
10117 Berlin 9494 Schaan
Germany Liechtenstein
Declaration number Declared product / declared unit
EPD-HIL-20230439-IBA1-EN The declared product is the MFT-FOX HI 300 M 11 as a representative
product for the MFT-FOX H and MFT-S2S portfolio. The declared unit is 1
kg of product. The packaging is also included in the calculation.
This declaration is based on the product category rules: Scope:
Building metals, 01/08/2021 This document relates to the MFT-FOX HI 300 M 11 as a representative
(PCR checked and approved by the SVR) product for the MFT-FOX H and the MFT-S2S products. FOX H and S2S
products cover the same applications and are very similar in material
constitution and therefore, have been summarized in this EPD.
Issue date Both portfolios can be divided into two classes per bracket size. The first
class contains the products without the isolator of Polypropylene and a
18/12/2023
pre-assembled screw. The second class contains the same products but
with an additional plastic part of polypropylene named isolator. The
declared product for this EPD is chosen from the second class, because it
Valid to
can be assumed that the environmental impacts are higher with the
17/12/2028 isolator and the steel screw that is included in the MFT-FOX H product line.
Moreover, FOX HI 300 M is chosen as a representative because it displays
the highest weight of the product group.
The owner of the declaration shall be liable for the underlying information
and evidence; the IBU shall not be liable with respect to manufacturer
information, life cycle assessment data and evidences.
The EPD was created according to the specifications of EN 15804+A2. In
the following, the standard will be simplified as EN 15804.
Verification
The standard EN 15804 serves as the core PCR
Dipl.-Ing. Hans Peters
Independent verification of the declaration and data according to ISO
(Chairman of Institut Bauen und Umwelt e.V.)
14025:2011
internally X externally
Florian Pronold Prof. Dr. Birgit Grahl,
(Managing Director Institut Bauen und Umwelt e.V.) (Independent verifier)
1 Environmental Product Declaration - Hilti AG - MFT FOX H & MFT S2S
Product
and horizontal support rails.
Product description/Product definition Product according to the CPR based on a hEN:
MFT-FOX HI and MFT FOX-S2S are designed as an aluminium For the placing on the market of the product in the European
substructure system. The brackets are suitable for all façade Union/European Free Trade Association (EU/EFTA) (with the
cladding. exception of Switzerland) Regulation (EU) No. 305/2011 (CPR)
The products are used for fastening ventilated façade applies. The product needs a declaration of performance taking
substructure to into consideration EN 1090-1:2009+A1:2011.
concrete, masonry, steel frame structure and wood. They
enable
mounting façade substructures on the primary structure
as a helping hand bracket and can be used to install vertical
2 Environmental Product Declaration - Hilti AG - MFT FOX H & MFT S2S
3 Environmental Product Declaration - Hilti AG - MFT FOX H & MFT S2S
movement against the brackets, while the flexible points allow
virtually frictionless sliding of the profiles against the brackets.
The flexible points make sure that there are no additional loads
on the substructure from the profile's expansion forces. With
Application this system, wall tolerances of up to 40 mm can be balanced.
MFT-FOX H & MFT-S2S are developed to be fixed on
base materials like concrete, masonry, steel frame structure Technical Data
and wood. This product is used as a substructure for ventilated Technical documentation according to EN 1090-3.
façade (rainscreen) applications. The brackets are supplied
Constructional data
with pre-assembled isolators and, according to the method of
Name Value Unit
installation to the base material – anchors, screws or direct
fastening can be used – with different hole geometries in the Thickness Baseplate 4 mm
base plate. The brackets are designed with both fixed and Length 60 -300 mm
flexible points to allow for thermal expansion of the profile. The Height 80 mm
fixed point takes the weight of the panels and substructure and
Width 62 mm
the proportional wind loads, while the flexible point only
Thickness Isolator 5 mm
assumes the proportional wind loads.
Performance data of the product in accordance with the
For MFT FOX H: declaration of performance with respect to its essential
During the application the horizontal profiles are connected to characteristics according to EN 1090- 1:2009+A1:2011
the brackets with specially designed screws, which combine the Standard for the execution of steel structures and aluminium
fixed and flexible points in one connection point. Due to thermal structures. The structural parts made of aluminium correspond
expansion of the profile the brackets take over this movement. to the following harmonized standards: EN 1090-1, DIN EN
1999-1-1 + DIN EN 1991-1-4 incl. national annexes, DIN
For MFT S2S: 18516-1. The product has a CE-marking Hilti MFT CPR-1346.
During the application the vertical profiles are connected to the
brackets with specially designed screws for fixed and flexible
points. The fixed points do not allow the profiles vertical
4 Environmental Product Declaration - Hilti AG - MFT FOX H & MFT S2S
exceeding 0.1 percentage by mass: no
Base materials/Ancillary materials
FOX H: Biocide products were added to this construction product or it
The raw material used for the production of this has been treated with biocide products (this then concerns a
product is aluminium alloy according to the treated product as defined by the Regulation on Biocide
standard EN AW-6063-T66 with 320g (92% of product weight). Products No. 528/2012): no
The alloy is a widely used extrusion alloy, suitable for various
applications. The material used for the isolator is polypropylene Packaging:
with 2g (6% of the product weight). The packaging of this product is carton. This cardboard
packaging can be recycled.
This product/article contains substances listed in the candidate
list exceeding 0.1 percentage by mass in accordance with Reference service life
Article 59(10) of the REACH Regulation: no The MFT-FOX H and MFT-S2S systems have a minimum
service life of 35 years when used as prescribed according to
This product/article/at least one partial article contains the BBA Certificate (British Board of Agreement). However, the
other carcinogenic, mutagenic, reprotoxic (CMR) substances in actual service life can be considerably longer.
categories 1A or 1B which are not on the candidate list,
LCA: Calculation rules
and Asia. The transport is carried out by lorry and ship. The
Declared Unit following flow charts illustrate the underlying production
The declared product here is an aluminium profile from HILTI process.
AG with the designation MFT Fox HI 300 M11 as a
representative product from the MFT Fox-H and MFT S2S
portfolio. It is the heaviest product with the additional screw in
the portfolio. The declared unit refers to 1 kg of aluminium
profile. The packaging, related to 1 kg aluminium profile, is
additionally included in the calculation with 0.0348 kg. The
following table shows the data of the declared unit.
Declared unit and mass reference
Name Value Unit
Declared unit 1 kg
Gross density 2.7 kg/m3
Figure Information modules A 1 to A3 of the product
System boundary
Type of EPD: Cradle to factory gate with options. The following
information modules are defined as system boundaries in this
study:
Production stage (A1- A3): Figure Information modules A 1 to A3 of the packaging
- A1, raw material extraction,
- A2, transport to the manufacturer,
- A3, production. In the information modules C1 to C4, the deconstruction or
demolition from the building, the transport to waste disposal,
the waste treatment and disposal of the product are recorded.
End of life (C1- C4): Furthermore, reuse, recovery and recycling potentials are
- C1, deconstruction/demolition, reported in information module D.
- C2, transport,
- C3, waste treatment ,
Geographic Representativeness
- C4, disposal.
Land or region, in which the declared product system is
manufactured, used or handled at the end of the product´s
lifespan: Europe
Reuse, recovery and recycling potential (D).
Comparability
In order to accurately capture the indicators and environmental
Basically, a comparison or an evaluation of EPD data is only
impacts of the declared unit, a total of 8 information modules
possible if all the data sets to be compared were created
are considered. The information modules A1 to A3 describe the
according to EN 15804 and the building context, respectively
material provision, the transport to the production site, as well
the product-specific characteristics of performance, are taken
as the production processes of the product itself.
into account. The database referred to in this study is LCA for
Experts by Sphera. (V1 2023)
The primary products are sourced from the European Union
LCA: Scenarios and additional technical information
5 Environmental Product Declaration - Hilti AG - MFT FOX H & MFT S2S
Name Value Unit
Characteristic product properties of biogenic carbon
Collected separately waste type waste type - kg
The declared product does not contain any biogenic
Collected as mixed construction waste 1 kg
Carbon.
Reuse - kg
Information on describing the biogenic carbon content at
Recycling 0.9565 kg
factory gate
Energy recovery 0.0435 kg
Name Value Unit
Landfilling - kg
Biogenic carbon content in accompanying kg
0.0037
packaging C
Reuse, recovery and/or recycling potentials (D), relevant
scenario information
In Module D, the metallic components are added to the primer
End of life (C1 - C4) material data sets through a recycling scenario of 85% and the
plastic components are thermally utilised, thereby generating
In information module C1, the demolition of the assembly
thermal and electrical energy.
system from the building is calculated. The demolition is carried
out by means of an electric screwdriver. The electrical energy Name Value Unit
consumption for the tool is assumed to be 0.012MJ for the Stainless Steel 0,024 kg
declared unit. The electricity consumption is calculated with a Aluminium 0,902 kg
European electricity mix.
6 Environmental Product Declaration - Hilti AG - MFT FOX H & MFT S2S
LCA: Results
DESCRIPTION OF THE SYSTEM BOUNDARY (X = INCLUDED IN LCA; ND = MODULE OR INDICATOR NOT DECLARED; MNR =
MODULE NOT RELEVANT)
Benefits and
Construction loads beyond
Product stage Use stage End-of-life stage
process stage the system
boundaries
la ire ta m w a Ry lp p u s tro p s n a rT g n iru tc a fu n a M e h t m o rf tro p s n a rTe tis e h t o t e ta g y lb m e s s A e s U e c n a n e tn ia M ria p e R tn e m e c a lp e R tn e m h s ib ru fe R y g re n e la n o ita re p Oe s u re ta w la n o ita re p Oe s u n o itc u rts n o c -e Dn o itilo m e d tro p s n a rT g n is s e c o rp e ts a W la s o p s iD -e s u e R-y re v o c e R-g n ilc y c e Rla itn e to p
A1 A2 A3 A4 A5 B1 B2 B3 B4 B5 B6 B7 C1 C2 C3 C4 D
X X X MND MND MND MND MNR MNR MNR MND MND X X X X X
RESULTS OF THE LCA - ENVIRONMENTAL IMPACT according to EN 15804+A2: 1 kg MFT FOX HI 300 M11
Parameter Unit A1-A3 C1 C2 C3 C4 D
Global Warming Potential total (GWP-total) kg CO 2 eq 1.03E+01 1.45E-03 7.81E-03 1.35E-01 0 -6.94E+00
Global Warming Potential fossil fuels (GWP-fossil) kg CO 2 eq 1.03E+01 1.45E-03 7.47E-03 1.35E-01 0 -6.94E+00
Global Warming Potential biogenic (GWP-biogenic) kg CO 2 eq 6.7E-03 7.23E-07 3.38E-04 0 0 -1.27E-03
Global Warming Potential luluc (GWP-luluc) kg CO 2 eq 3.34E-03 1.33E-07 4.7E-07 1.94E-05 0 -1.83E-03
Depletion potential of the stratospheric ozone layer (ODP) kg CFC11 eq 1.34E-11 1.43E-14 8.82E-16 1.05E-14 0 -9.51E-12
Acidification potential of land and water (AP) mol H+ eq 4.58E-02 2.21E-06 8.82E-06 2.64E-05 0 -3.19E-02
Eutrophication potential aquatic freshwater (EP-freshwater) kg P eq 8.32E-06 1.44E-09 1.81E-09 1.02E-08 0 -4.05E-06
Eutrophication potential aquatic marine (EP-marine) kg N eq 6.97E-03 6.23E-07 3.15E-06 8.85E-06 0 -4.65E-03
Eutrophication potential terrestrial (EP-terrestrial) mol N eq 7.58E-02 6.59E-06 3.56E-05 1.29E-04 0 -5.06E-02
Formation potential of tropospheric ozone photochemical oxidants kg NMVOC
2.1E-02 1.72E-06 8.34E-06 2.47E-05 0 -1.41E-02
(POCP) eq
Abiotic depletion potential for non fossil resources (ADPE) kg Sb eq 5.94E-06 7.03E-11 9.25E-11 2.79E-09 0 -4.81E-06
Abiotic depletion potential for fossil resources (ADPF) MJ 1.39E+02 3.19E-02 1.07E-01 6.6E-02 0 -9.25E+01
m3 world eq
Water use (WDP) 1.46E+00 1.22E-04 1.8E-05 1.27E-02 0 -1.03E+00
deprived
RESULTS OF THE LCA - INDICATORS TO DESCRIBE RESOURCE USE according to EN 15804+A2: 1 kg MFT FOX HI 300 M11
Parameter Unit A1-A3 C1 C2 C3 C4 D
Renewable primary energy as energy carrier (PERE) MJ 5.73E+01 4.37E-03 6.93E-04 8.68E-03 0 -4.05E+01
Renewable primary energy resources as material utilization
MJ 5.2E-01 0 0 0 0 0
(PERM)
Total use of renewable primary energy resources (PERT) MJ 5.73E+01 4.37E-03 6.93E-04 8.68E-03 0 -4.05E+01
Non renewable primary energy as energy carrier (PENRE) MJ 1.4E+02 3.19E-02 1.08E-01 6.61E-02 0 -9.27E+01
Non renewable primary energy as material utilization (PENRM) MJ 0 0 0 0 0 0
Total use of non renewable primary energy resources (PENRT) MJ 1.4E+02 3.19E-02 1.08E-01 6.61E-02 0 -9.27E+01
Use of secondary material (SM) kg 3.83E-02 0 0 0 0 0
Use of renewable secondary fuels (RSF) MJ 0 0 0 0 0 0
Use of non renewable secondary fuels (NRSF) MJ 0 0 0 0 0 0
Use of net fresh water (FW) m3 1.36E-01 7.31E-06 8.05E-07 3E-04 0 -9.61E-02
RESULTS OF THE LCA – WASTE CATEGORIES AND OUTPUT FLOWS according to EN 15804+A2:
1 kg MFT FOX HI 300 M11
Parameter Unit A1-A3 C1 C2 C3 C4 D
Hazardous waste disposed (HWD) kg 1.04E-08 1.85E-12 1.98E-13 2.23E-13 0 -5.91E-09
Non hazardous waste disposed (NHWD) kg 2.71E+00 7.03E-06 1.07E-05 5.37E-04 0 -1.93E+00
Radioactive waste disposed (RWD) kg 7.98E-03 4.97E-06 1.8E-07 1.62E-06 0 -5.71E-03
Components for re-use (CRU) kg 0 0 0 0 0 0
Materials for recycling (MFR) kg 0 0 0 0 0 0
Materials for energy recovery (MER) kg 0 0 0 0 0 0
Exported electrical energy (EEE) MJ 0 0 0 0 0 0
Exported thermal energy (EET) MJ 0 0 0 0 0 0
RESULTS OF THE LCA – additional impact categories according to EN 15804+A2-optional:
1 kg MFT FOX HI 300 M11
Parameter Unit A1-A3 C1 C2 C3 C4 D
Disease
Incidence of disease due to PM emissions (PM) ND ND ND ND ND ND
incidence
Human exposure efficiency relative to U235 (IR) kBq U235 eq ND ND ND ND ND ND
Comparative toxic unit for ecosystems (ETP-fw) CTUe ND ND ND ND ND ND
Comparative toxic unit for humans (carcinogenic) (HTP-c) CTUh ND ND ND ND ND ND
Comparative toxic unit for humans (noncarcinogenic) (HTP-nc) CTUh ND ND ND ND ND ND
7 Environmental Product Declaration - Hilti AG - MFT FOX H & MFT S2S
Soil quality index (SQP) SQP ND ND ND ND ND ND
Disclaimer 1 – for the indicator “Potential Human exposure efficiency relative to U235”. This impact category deals mainly with the
eventual impact of low-dose ionizing radiation on human health of the nuclear fuel cycle. It does not consider effects due to possible
nuclear accidents, occupational exposure or radioactive waste disposal in underground facilities. Potential ionizing radiation from the
soil, radon and from some construction materials is also not measured by this indicator.
Disclaimer 2 – for the indicators “abiotic depletion potential for non-fossil resources”, “abiotic depletion potential for fossil resources”,
“water (user) deprivation potential, deprivation-weighted water consumption”, “potential comparative toxic unit for ecosystems”,
“potential comparative toxic unit for humans – cancerogenic”, “Potential comparative toxic unit for humans - not cancerogenic”,
“potential soil quality index”. The results of this environmental impact indicator shall be used with care as the uncertainties on these
results are high as there is limited experience with the indicator.
References
on EU Biocidal Products
DIN EN 1090-1
Standard for execution of steel structures and aluminium Other references
structures
BBA Certificate (British Board of Agrément)
DIN EN 1999-1-1 + DIN EN 1991-1-4 The British Board of Agrément is a UK body issuing certificates
Eurocode 9: Design of aluminum structures - Part 1-4: General for construction products and systems and providing inspection
design rules services in support of their designers and installers.
DIN 18516-1 Calculation rules: PCR - Part A
Product category rules for construction products and services -
DIN 18516-1:2010-06 Cladding for external walls, ventilated at Calculation rules for the eco-balance and requirements for the
rear facades – Part 1: Requirements, princicples of testing background report V1.3, Institut Bauen und Umwelt e.V.,
08.2022.
EN 1090-1:2009+A1:2011
Standard for execution of steel structures and aluminium CML 2001 April. 2015
structures Indicators for environmental impacts, Leiden: Universität
Leiden,
EN AW-6063-T66 http://cml.leiden.edu/software/datacmlia.
Type of aluminium alloy html#downloads (20.08.2022)
EN 15804 IBU 2021
EN 15804:2012+A2:2019+AC:2021, Sustainability General Instructions for the EPD programme of Institut Bauen
ofconstruction works — Environmental Product Declarations — und Umwelt e.V. Version 2.0,
Core rules for the product category of construction products. Berlin: Institut Bauen und Umwelt e.V., 2021
www.ibu-epd.de
ISO 14025
DIN EN /ISO 14025:2011-10/, Environmental labels and Product category rules for construction products – Part B
declarations — Type III environmental Institut Bauen und Umwelt e.V, Berlin (pub.): Product Category
declarations — Principles and procedures Rules for Construction Products from the range
ofEnvironmental Product Declarations for Institut Bauen und
Regulation (EU) No. 305/2011 Umwelt (IBU), PConstruction metals ,.01.08.2021
Construction Product Regulation (CPR)
Sphera
Regulation (EC) No 1907/2006 LCA for Experts: Ganzheitliche Bilanzierung Leinfelden-
REACH Regulation Echterdingen; Sphera Solution GmbH (Hrsg.)
www.gabi-software.com/deutsch/index/
Regulation (EU) No 528/2012 (27.06.2023)
8 Environmental Product Declaration - Hilti AG - MFT FOX H & MFT S2S
Publisher
Institut Bauen und Umwelt e.V. +49 (0)30 3087748- 0
Hegelplatz 1 info@ibu-epd.com
10117 Berlin www.ibu-epd.com
Germany
Programme holder
Institut Bauen und Umwelt e.V. +49 (0)30 3087748- 0
Hegelplatz 1 info@ibu-epd.com
10117 Berlin www.ibu-epd.com
Germany
Author of the Life Cycle Assessment
FIT-Umwelttechnik GmbH 05362 72 69 474
Westerstr. 13 bertram@fit-umwelttechnik.de
38442 Wolfsburg www.fit-umwelttechnik.com
Germany
Owner of the Declaration
Hilti Aktiengesellschaft +423 234 2111
Feldkircher Strasse 100 HAGHSE@hilti.com
9494 Schaan www.hilti.com
Liechtenstein
9 Environmental Product Declaration - Hilti AG - MFT FOX H & MFT S2S
