Environmental product declaration
in accordance with ISO 14025 and EN 15804+A2
Microdol 5
Owner of the declaration: Program operator:
Omya Hustadmarmor AS The Norwegian EPD Foundation
Product: Declaration number:
Microdol 5
NEPD-7287-6687-EN
Declared unit:
1 tonne Registration number:
This declaration is based on Product Category Rules: NEPD-7287-6687-EN
CEN Standard EN 15804:2012+A2:2019 serves as core
Issue date: 21.08.2024
PCR
The Norwegian EPD Foundation
NPCR Part A: Construction products and services. Ver. 2.0 Valid to: 21.08.2029
March 2021
EPD software:
LCAno EPD generator ID: 470848
1 / 11
General information
Product Owner of the declaration:
Microdol 5 Omya Hustadmarmor AS
Contact person: Lovise Stakvik
Phone: +47 41322610
e-mail: lovise.stakvik@omya.com
Program operator: Manufacturer:
The Norwegian EPD Foundation Omya Hustadmarmor AS
Post Box 5250 Majorstuen, 0303 Oslo, Norway Sjøvegen 69
Phone: +47 977 22 020 6440 Elnesvågen, Norway
web: www.epd-norge.no
Declaration number: Place of production:
Omya Hustadmarmor AS, production site Knarrevik
NEPD-7287-6687-EN
Langebakken 31
5355 Knarrevik, Norway
This declaration is based on Product Category Rules: Management system:
CEN Standard EN 15804:2012+A2:2019 serves as core PCR 9001, 14001, 45001, and 50001
NPCR Part A: Construction products and services. Ver. 2.0 March
2021
Statement of liability: Organisation no:
The owner of the declaration shall be liable for the underlying 912864227
information and evidence. EPD Norway shall not be liable with respect
to manufacturer information, life cycle assessment data and
evidences.​
Declared unit: Issue date:
1 tonne Microdol 5 21.08.2024
Declared unit (cradle to gate) with option: Valid to:
A1-A3,A4 21.08.2029
Year of study:
2023
Functional unit: Comparability:
Not applicable. EPD of construction products may not be comparable if they not
comply with EN 15804 and seen in a building context.
General information on verification of EPD from EPD tools: Development and verification of EPD:
Independent verification of data, other environmental information The declaration is created using EPD tool lca.tools ver EPD2022.03,
and the declaration according to ISO 14025:2010, § 8.1.3 and § 8.1.4. developed by LCA.no. The EPD tool is integrated in the company's
Verification of each EPD is made according to EPD-Norway’s management system, and has been approved by EPD Norway.
guidelines for verification and approval requiring that tools are i)
integrated into the company's environmental management system, ii) Developer of EPD: Pedro Ferreira
the procedures for use of the EPD tool are approved by EPD-Norway,
Reviewer of company-specific input data and EPD: Børge Heggen
and iii) the process is reviewed annually by an independent third
Johansen, Energiråd AS
party verifier. See Appendix G of EPD-Norway's General Programme
Instructions for further information on EPD tools
Verification of EPD tool: Approved:
Independent third party verification of the EPD tool, background data
and test-EPD in accordance with EPDNorway's procedures and
guidelines for verification and approval of EPD tools.
Third party verifier:
VERIFIER NAME
(no signature required)
2 / 11
Product
Product description:
Fine, white dolomite powder, high purity and low binder absorption. The product is delivered in bulk, and therefore has no packaging.
Applications:
Paints, emulsion paints, heavy-duty coatings, road-marking paints plastics, plasticized PVC, polyester moldings, polymer concrete, adhesives,
sealants, fiberglass, lake and river liming, among others.
Product specification
Composition: Calcium magnesium carbonate (CaMg(CO3)2) - 99%, HCl (insoluble content) - 1%
Materials Value Unit
Stone 1000 kg
Technical data:
For technical information, contact at https://www.omya.com/en
Market:
Norway and Europe.
Reference service life, product
Not applicable.
Reference service life, building
Not applicable.
LCA: Calculation rules
Declared unit:
1 tonne Microdol 5
Cut-off criteria:
All major raw materials and all the essential energy is included. The production processes for raw materials and energy flows with very small
amounts (less than 1%) are not included. These cut-off criteria do not​ apply for hazardous materials and substances.
Allocation:
The allocation is made in accordance with the provisions of EN 15804. Incoming energy and water and waste production in-house is allocated
equally among all products through mass allocation. Effects of primary production of recycled materials is allocated to the main product in which
the material was used. The recycling process and transportation of the material is allocated to this analysis.
Data quality:
Specific data for the product composition are provided by the manufacturer. They represent the production of the declared product and were
collected for EPD development in the year of study. Background data is based on registered EPDs according to EN 15804, Ostfold Research
databases, ecoinvent and other LCA databases. The data quality of the raw materials in A1 is presented in the table below.​
Materials Source Data quality Year
Natural stone Supplier specific Supplier specific 2023
3 / 11
System boundaries (X=included, MND=module not declared, MNR=module not relevant)
Construction Beyond the system
Product stage Use stage End of life stage
installation stage boundaries
A1 A2 A3 A4 A5 B1 B2 B3 B4 B5 B6 B7 C1 C2 C3 C4 D
X X X X MND MND MND MND MND MND MND MND MND MND MND MND MND
System boundary:
The system includes the extraction of stone at Omya Hustadmarmor AS: Hammerfall (module A1), the transport of the stone by boat to Knarrevik
(module A2), the manufacturing of Microdol 5 (module A3), and its distribution to clients (module A4).
Additional technical information:
Not applicable.
waR slairetam tropsnarT gnirutcafunaM tropsnarT ylbmessA e​sU ecnanetniaM riapeR tnemecalpeR tnemhsibrufeR lanoitarepO ygrene esu lanoitarepO esu retaw -eD noitcurtsnoc noitilomed tropsnarT etsaW gnissecorp lasopsiD -yrevoceR-esueR laitnetop-gnilcyceR
4 / 11
LCA: Scenarios and additional technical information
The following information describe the scenarios in the different modules of the EPD.
Module A4 contains an average distance of transportation to the Norwegian market, with a truck of capacity higher than 32 tonnes.
Modules C and D are not relevant for this product, as it fulfills the three criteria described by EN 15804+A2:2019, namely: 1) the product is
physically integrated with other materials during installation so it cannot be physically retrieved at end of life; 2) The product is no longer
identifiable at end of life as a result of a physical or chemical transformation process; and 3) The product does not contain biogenic carbon.
Capacity utilisation Value
Transport from production place to user (A4) Distance (km) Fuel/Energy Consumption Unit
(incl. return) % (Liter/tonne)
Truck, over 32 tonnes, EURO 6 (km) - Europe 53,3 % 100 0,023 l/tkm 2,30
5 / 11
LCA: Results
The LCA results are presented below for the declared unit defined on page 2 of the EPD document.
Environmental impact
Indicator Unit A1-A3 A4
GWP-total kg CO2 -eq 4,01E+01 8,72E+00
GWP-fossil kg CO2 -eq 3,99E+01 8,71E+00
GWP-biogenic kg CO2 -eq 1,83E-01 3,73E-03
GWP-luluc kg CO2 -eq 2,85E-02 2,65E-03
ODP kg CFC11 -eq 6,97E-06 2,10E-06
AP mol H+ -eq 1,01E+00 2,80E-02
EP-FreshWater kg P -eq 4,52E-04 6,93E-05
EP-Marine kg N -eq 2,35E-01 6,14E-03
EP-Terrestial mol N -eq 2,63E+00 6,85E-02
POCP kg NMVOC -eq 6,81E-01 2,69E-02
ADP-minerals&metals1 kg Sb-eq 4,55E-04 1,55E-04
ADP-fossil1 MJ 5,19E+02 1,41E+02
WDP1 m3 1,19E+04 1,08E+02
GWP-total = Global Warming Potential total; GWP-fossil = Global Warming Potential fossil fuels; GWP-biogenic = Global Warming Potential biogenic; GWP-luluc =
Global Warming Potential land use and land use change; ODP = Depletion potential of the stratospheric ozone layer; AP = Acidification potential, Accumulated
Exceedance; EP-freshwater = Eutrophication potential, fraction of nutrients reaching freshwater end compartment: EP-marine = Eutrophication potential, fraction of
nutrients reaching marine end compartment; EP-terrestrial = Eutrophication potential, Accumulated Exceedance; POCP = Formation potential of tropospheric ozone;
ADP-minerals&metals = Abiotic depletion potential for non-fossil resources; ADP-fossil = Abiotic depletion for fossil resources potential; WDP = Water (user)
deprivation potential, deprivation-weighted water consumption
"Reading example: 9,0 E-03 = 9,0*10-3 = 0,009"
*INA Indicator Not Assessed
1. The results of this environmental impact indicator shall be used with care as the uncertainties on these results are high or as there is limited experienced with the
indicator
Remarks to environmental impacts
6 / 11
Additional environmental impact indicators
Indicator Unit A1-A3 A4
PM Disease incidence ND ND
IRP2 kgBq U235 -eq ND ND
ETP-fw1 CTUe ND ND
HTP-c1 CTUh ND ND
HTP-nc1 CTUh ND ND
SQP1 dimensionless ND ND
PM = Particulate Matter emissions; IRP = Ionizing radiation – human health; ETP-fw = Eco toxicity – freshwater; HTP-c = Human toxicity – cancer effects; HTP-nc =
Human toxicity – non cancer effects; SQP = Soil Quality (dimensionless)
"Reading example: 9,0 E-03 = 9,0*10-3 = 0,009"
*INA Indicator Not Assessed
1. The results of this environmental impact indicator shall be used with care as the uncertainties on these results are high or as there is limited experienced with the
indicator
2. This impact category deals mainly with the eventual impact of low dose ionizing radiation on human health of the nuclear fuel cycle. It does not consider effects due
to possible nuclear accidents, occupational exposure nor due to radioactive waste disposal in underground facilities. Potential ionizing radiation from the soil, from
radon and from some construction materials is also not measured by this indicator.
7 / 11
Resource use
Indicator Unit A1-A3 A4
PERE MJ 8,78E+02 1,78E+00
PERM MJ 3,20E-03 0,00E+00
PERT MJ 8,78E+02 1,78E+00
PENRE MJ 5,18E+02 1,41E+02
PENRM MJ 1,23E+00 0,00E+00
PENRT MJ 5,20E+02 1,41E+02
SM kg 0,00E+00 0,00E+00
RSF MJ 7,69E-01 6,23E-02
NRSF MJ 2,13E+00 2,09E-01
FW m3 6,58E+00 1,61E-02
PERE = Use of renewable primary energy excluding renewable primary energy resources used as raw materials; PERM = Use of renewable primary energy resources used
as raw materials; PERT = Total use of renewable primary energy resources; PENRE = Use of non renewable primary energy excluding non-renewable primary energy
resources used as raw materials; PENRM = Use of non renewable primary energy resources used as raw materials; PENRT = Total use of non renewable primary energy
resources; SM = Use of secondary materials; RSF = Use of renewable secondary fuels; NRSF = Use of non-renewable secondary fuels; FW = Net use of fresh water
"Reading example: 9,0 E-03 = 9,0*10-3 = 0,009"
*INA Indicator Not Assessed
8 / 11
End of life - Waste
Indicator Unit A1-A3 A4
HWD kg 2,67E-01 7,74E-03
NHWD kg 5,96E+00 1,23E+01
RWD kg 3,84E-03 9,66E-04
HWD = Hazardous waste disposed; NHWD = Non-hazardous waste disposed; RWD = Radioactive waste disposed
"Reading example: 9,0 E-03 = 9,0*10-3 = 0,009"
*INA Indicator Not Assessed
End of life - Output flow
Indicator Unit A1-A3 A4
CRU kg 0,00E+00 0,00E+00
MFR kg 1,23E-02 0,00E+00
MER kg 3,62E-01 0,00E+00
EEE MJ 2,06E-01 0,00E+00
EET MJ 3,12E+00 0,00E+00
CRU = Components for re-use; MFR = Materials for recycling; MER = Materials for energy recovery; EEE = Exported energy electrical; EET = Exported energy thermal
"Reading example: 9,0 E-03 = 9,0*10-3 = 0,009"
*INA Indicator Not Assessed
Biogenic Carbon Content
Indicator Unit At the factory gate
Biogenic carbon content in product kg C 0,00E+00
Biogenic carbon content in accompanying packaging kg C 0,00E+00
Note: 1 kg biogenic carbon is equivalent to 44/12 kg CO2
9 / 11
Additional requirements
Greenhouse gas emissions from the use of electricity in the manufacturing phase
National production mix from import, low voltage (production of transmission lines, in addition to direct emissions and losses in grid) of applied
electricity for the manufacturing process (A3).
Electricity mix Source Amount Unit
Electricity, Norway (kWh) ecoinvent 3.6 24,33 g CO2-eq/kWh
Dangerous substances
The product contains no substances given by the REACH Candidate list.
Indoor environment
Additional Environmental Information
Additional environmental impact indicators required in NPCR Part A for construction products
Indicator Unit A1-A3 A4
GWPIOBC kg CO2 -eq 4,00E+01 8,72E+00
GWP-IOBC: Global warming potential calculated according to the principle of instantaneous oxidation. In order to increase the transparency of biogenic carbon​
contribution to climate impact, the indicator GWP-IOBC is required as it declares climate impacts calculated according to the principle of instantaneous oxidation.​
GWP-IOBC is also referred to as GWP-GHG in context to Swedish public procurement legislation.
10 / 11
Bibliography
ISO 14025:2010 Environmental labels and declarations - Type III environmental declarations - Principles and procedures.
ISO 14044:2006 Environmental management - Life cycle assessment - Requirements and guidelines.
EN 15804:2012+A2:2019 Environmental product declaration - Core rules for the product category of construction products.
ISO 21930:2017 Sustainability in buildings and civil engineering works - Core rules for environmental product declarations of construction
products.
ecoinvent v3, Allocation, cut-off by classification, Swiss Centre of Life Cycle Inventories.
Iversen et al., (2018 eEPD v3.0 - Background information for EPD generator system. LCA.no report number 04.18.
Ruttenborg et al., (2022 EPD generator for NPCR022:2022 - Background information for EPD generator application and LCA data, LCA.no report
number xx.22
NPCR Part A: Construction products and services. Ver. 2.0. March 2021, EPD-Norge.
Program operator and publisher Phone: +47 977 22 020
The Norwegian EPD Foundation e-mail: post@epd-norge.no
Post Box 5250 Majorstuen, 0303 Oslo, Norway web: www.epd-norge.no
Owner of the declaration: Phone: +47 41322610
Omya Hustadmarmor AS e-mail: lovise.stakvik@omya.com
Sjøvegen 69, 6440 Elnesvågen web: www.omya.com
Author of the Life Cycle Assessment Phone: +47 916 50 916
LCA.no AS e-mail: post@lca.no
Dokka 6A, 1671 web: www.lca.no
Developer of EPD generator Phone: +47 916 50 916
LCA.no AS e-mail: post@lca.no
Dokka 6B,1671 Kråkerøy web: www.lca.no
ECO Platform web: www.eco-platform.org
ECO Portal web: ECO Portal
11 / 11
