ENVIRONMENTAL PRODUCT DECLARATION
as per ISO 14025 and EN 15804+A2
Owner of the Declaration FEICA, EFCC, IVK, DBC
Programme holder Institut Bauen und Umwelt e.V. (IBU)
Publisher Institut Bauen und Umwelt e.V. (IBU)
Declaration number EPD-DBC-20220218-IBF1-EN
Issue date 26.09.2022
Valid to 25.09.2027
Modified mineral mortars, group 2
FEICA - Association of the European Adhesive and Sealant Industry
EFCC - European Federation for Construction Chemicals
IVK - Industrieverband Klebstoffe e.V.
DBC - Deutsche Bauchemie e.V.
www.ibu-epd.com | https://epd-online.com
Umwelt Produktdeklaration Name des Herstellers – Name des Produkts
1. General Information
DBC - Deutsche Bauchemie e.V.
EFCC - European Federation for Modified mineral mortars, group 2
Construction Chemicals
FEICA - Association of the European
Adhesive and Sealant Industry
IVK - Industrieverband Klebstoffe e.V.
Programme holder Owner of the declaration
IBU – Institut Bauen und Umwelt e.V. DBC, Mainzer Landstr. 55, D-60329 Frankfurt a.M.
Hegelplatz 1 EFCC, 172 Boulevard du Triomphe, B-1160 Brussels
10117 Berlin FEICA, Rue Belliard 40, B-1040 Brussels
Germany IVK, Völklingerstr. 4, D-40219 Düsseldorf
Declaration number Declared product / declared unit
EPD-DBC-20220218-IBF1-EN 1 kg of modified mineral mortar with a density 800 -
1,700 kg/m³
This declaration is based on the product Scope:
category rules: This verified EPD entitles the holder to bear the
Mineral factory-made mortar, 11.2017 symbol of the Institut Bauen und Umwelt e.V. It
(PCR checked and approved by the SVR) exclusively applies to products produced in Europe and
for a period of five years from the date of issue. This
EPD may be used by members of FEICA, EFCC, DBC
Issue date
and IVK and their members provided it has been
26.09.2022
proven that the respective product can be represented
by this EPD. For this purpose, a guideline is available
Valid to at the secretariats of the four associations. The
25.09.2027 members of the associations are listed on their
respective websites.
The owner of the declaration shall be liable for the
underlying information and evidence; the IBU shall not
be liable with respect to manufacturer information, life
cycle assessment data and evidences.
The EPD was created according to the specifications
of EN 15804+A2. In the following, the standard will be
simplified as EN 15804.
Verification
The standard EN 15804 serves as the core PCR
Independent verification of the declaration and data
according to ISO 14025:2011
Dipl. Ing. Hans Peters internally x externally
(chairman of Institut Bauen und Umwelt e.V.)
Dr. Alexander Röder Matthias Schulz
(Managing Director Institut Bauen und Umwelt e.V.)) (Independent verifier)
2. Product
2.1 Product description/Product definition For the placing on the market in the European
Modified mineral mortars are combinations of one or Union/European Free Trade Association (EU/EFTA)
more inorganic binders, fillers, aqueous dispersions or with the exception of Switzerland) products falling
dispersion powders, water and if necessary additives. under the Regulation (EU) No 305/2011 (CPR) need a
They comply with manifold, often specific, functions in Declaration of Performance taking into consideration
the construction, furnishing and refurbishment of either the relevant harmonised European standard or
buildings. The product displaying the highest the European Technical Assessment and the CE
environmental impacts was used as a representative marking. For the application and use of the products
product for calculating the Life Cycle Assessment the respective national provisions apply.
results (worst-case approach).
2 Environmental Product Declaration DBC, EFCC, FEICA, IVK – Modified mineral mortar, group 2
2.2 Application Module 1: Modified mineral mortars as repair
Modified mineral mortars are used for the following mortar for the protection and repair of concrete
applications: structures
1.1 Products used to restore and/or replace defective
Module 1: Modified mineral mortars as repair concrete
mortar for the protection and repair of concrete The requirements on essential characteristics for all
structures intended uses in accordance with EN 1504­3, Tables 1
1.1 Products used to restore and/or replace defective and 3, must be maintained. These are:
concrete - Compressive strength (EN 12190)
1.2 Products to protect reinforcement, necessary to - Chloride ion content (EN 1015­17)
extend the service life of a concrete structure exhibiting - Adhesive strength by pull-off test (EN 1542)
deterioration
1.2 Products to protect reinforcement
Module 2: Adhesives based on modified mineral The requirements on essential characteristics for all
mortars intended uses in accordance with EN 1504­7, Table 1,
2.1 Products for bonding ceramic tiles as well as must be maintained. This is
natural stone for internal and external installations on - Corrosion protection (EN 15183)
walls, floors and ceilings Further essential characteristics in accordance with the
2.2 Products for bonding thermal insulation composite manufacturer's technical documentation/declaration of
panels performance
Module 3: Modified mineral mortars as joint fillers Module 2: Adhesives based on modified mineral
Products for joint filling of wall and floor coverings mortars
made of ceramic tiles as well as natural stone for 2.1 Products for bonding ceramic tiles as well as
indoor and outdoor applications natural stone for internal and external installations on
walls, floors and ceilings
Module 4: Modified mineral mortars as screed, The requirements on essential characteristics
floor levelling compounds, fillers, flowing screed according to EN 12004, Table 1, must be maintained.
Products for screed/synthetic resin screed for use in These are:
floor constructions - Tensile adhesion strength after dry storage (EN
12004­2)
Module 5: Modified mineral mortars as levelling - Tensile adhesion strength after water immersion (EN
compounds for walls and ceilings 12004­2)
Products for levelling and repairing rough, uneven - Tensile adhesion strength after heat ageing (EN
walls, for repairing grit spots, closing blowholes and 12004­2)
modelling broken corners and edges - Tensile adhesion strength after freeze/thaw cycles
(EN 12004­2)
Module 6: Modified mineral mortars as grouts - Open time: Tensile strength (EN 12004­2)
Products for grouting on holes, recesses, concrete Further essential characteristics in accordance with the
precast columns, foundations and for anchoring manufacturer's technical documentation/declaration of
machine components indoors and outdoors performance
2.2 The minimum requirement of EAD 040083­00­0404
Module 7: Modified mineral mortars for liquid External Thermal Insulation Composite Systems with
applied products for waterproofing of buildings Rendering must be maintained. The essential
Products for providing cement-based waterproofing characteristics are to be specified in accordance with
surfaces in structural and civil engineering. For use in the European technical assessment (ETA,
new and old buildings as well as beneath tiles specification no.). Further essential characteristics in
7.1 Liquid-applied water impermeable products for use accordance with the manufacturer's technical
beneath ceramic tiling documentation/declaration of performance
7.2 Products for waterproofing with mineral
waterproofing slurries or flexible polymer modified thick Module 3: Modified mineral mortars as joint fillers
coatings The minimum requirements of EN 13888 must be
7.3 Products for water proofing in conjunction with maintained.
ceramic tiles
7.4 Products for waterproofing with flexible polymer Module 4: Modified mineral mortars as screed,
modified mineral thick coatings floor levelling compounds, fillers, flowing screed
The requirements on essential characteristics
Module 8: Modified mineral mortars for according to EN 13813 ‘Screed material and floor
waterproofing floors and/or walls inside buildings screeds – Screed materials – Properties and
Products for watertight covering in wet rooms inside requirements’ must be maintained. For synthetic resin
buildings screeds, these are:
- Bond strength (EN 13892­8)
2.3 Technical Data - Reaction to fire (EN 13501­1)
The density of the products is between 0,80 and 1,70 Further essential characteristics in accordance with the
g/cm³, other relevant technical data can be found in the manufacturer's technical documentation/declaration of
manufacturer’s technical documentation. performance
Construction products with Declaration of Performance
in accordance with CPR and the manufacturer's Module 5: Modified mineral mortars as levelling
technical documentation: compounds for walls and ceilings
Module 5.1: The minimum requirements of EN 998­1
apply. These are: - Reaction to fire (EN 13501­1) -
3 Environmental Product Declaration DBC, EFCC, FEICA, IVK – Modified mineral mortar, group 2
Compressive strength - Dry bulk density - Capillary
water absorption - Water vapour permeability
Further essential characteristics in accordance with the
manufacturer's technical documentation/declaration of
performance 2.4 Delivery status
Module 5.2: The minimum requirements of EN 13279 Modified mineral mortars are generally manufactured
apply. Further essential characteristics in accordance and supplied as factory-made dry mortars. Factory-
with the manufacturer's technical made dry mortar is a finished mixture of base materials
documentation/declaration of performance which merely requires the addition of water and/or a
polymer dispersion on the building site. The products
Module 6: Modified mineral mortars as grouts can be supplied in 1-5 kg bags, 15-25 kg sacks, big
The requirements of DAfStb Guideline on 'Production bags (1 t), minitainers (1.2 t) or as silo goods (5-15 t).
and use of cement-bound flow concrete and grouting Paper sacks with polyethylene lining were modelled as
mortar' (VeBMR) must be maintained. packaging (worst-case approach).
The requirements according to MVV TB No. C 2.1.4.5
for "Ü-mark" must be maintained. 2.5 Base materials/Ancillary materials
Typically, the products covered by this EPD contain
Module 7: Modified mineral mortars for liquid the following range of base materials and auxiliaries
applied products for waterproofing of buildings (% by mass):
7.1 Inorganic binder: ~ 2 - 98
The requirements according to EN 14891 , table 1, Filler materials: ~ 0 - 90
must be maintained. These are: Additives: ~ 0 - 10
- initial tensile adhesion strength EN 14891 Aqueous dispersion and/or dispersion powder: ~ 0 -
- Tensile adhesion strength after water contact EN 35
14891
- Waterproofing EN 14891 These ranges are average values and the composition
- Crack bridging ability EN 14891 of products complying with the EPD can deviate from
7.2 these concentration levels in individual cases. More
The minimum requirements of the 'Testing principles detailed information is available in the respective
for granting general building authority approved test manufacturer's documentation (e.g. product data
certificates for waterproofing with mineral sheets).
waterproofing slurries and flexible polymer modified Note: For companies to declare their products within
thick coatings' (PG MDS/FPD) must be maintained. the scope of this EPD it is not sufficient to simply
The characteristics for the proof of usability are to be comply with the product composition shown above.
specified in accordance with the test principles for The application of this EPD is only possible for
granting general building authority test certificates for member companies of DBC, EFCC, FEICA, and IVK
waterproofing with mineral waterproofing slurries and member associations and only for specific formulations
flexible polymer thick coatings. with a total score below the declared maximum score
7.3 for a product group according to the associated
The minimum requirements of the 'testing principles for guidance document.
granting general building authority approved test
certificates for waterproofing in conjunction with
ceramic tiles' (PG AIV) must be considered. 1. substances from the “Candidate List of
7.4 Substances of Very High Concern for
The minimum requirement of EAD 030295­00­ Authorisation” (SVHC)
0605 must be maintained. The essential characteristics If this product contains substances listed in the
are to be specified in accordance with the European candidate list (latest version) exceeding 0.1
technical assessment (ETA, specification no.). percentage by mass, the relevant information can be
found in the safety data sheet of the relevant product
Module 8: Modified mineral mortars for covered by this model EPD.
waterproofing floors and/or walls inside buildings 2. CMR substances in categories 1A and 1B
The minimum requirement of EAD 030352­00­ If this product contains other carcinogenic, mutagenic,
0503 must be maintained. The essential characteristics reprotoxic (CMR) substances in categories 1A or 1B
are to be specified in accordance with the European which are not on the candidate list, exceeding 0.1
technical assessment (ETA, specification no.). percentage by mass, the relevant information can be
found in the safety data sheet of the relevant product
covered by this model EPD.
3. Biocide products added to the construction
Constructional data product
Name Value Unit If this construction product contains biocide products,
Compressive strength - N/mm2 the active substances, information on the
Adhesive shear strength - N/mm2 concentration and/or concentration range, the product
Water absorption - mg type together with information on their hazardous
Water vapor diffusion equivalent air properties are listed in the safety data sheet of the
- m
layer thickness respective product.
Thermal conductivity - W/(mK)
Tensile bond strength - N/mm2
Flexural strength - N/mm2 2.6 Manufacture
The raw materials are stored in silos, big bags or sacks
Sound absorption coefficient (if
- % in the manufacturing plant and fed gravimetrically in
relevant)
4 Environmental Product Declaration DBC, EFCC, FEICA, IVK – Modified mineral mortar, group 2
accordance with the respective formula and mixed designated purpose of the respective products. It is a
intensively. The mix is then packaged. durable product which, when used as adhesive,
screed, waterproofing material or repair product,
2.7 Environment and health during makes an essential contribution towards improving
manufacturing building function and value.
The state of the art involves maximum recirculation of
dry waste into production. Wherever dust is incurred 2.11 Environment and health during use
during production in the plant, it is directed to a filter Owing to the stable crystalline bond and firm structure
system considering the limit values applicable for the achieved after curing, emissions are extremely low and
workplace and using the corresponding extraction harmless to health when the respective products are
plants. Sack discharge stations connected to the used in accordance with the designated purpose. No
extraction plant offer employees additional protection risks are known for water, air and soil if the products
from dust. Most of the dust collected in the filter system are used as designated. Natural ionising radiation from
and any residue incurred during production is returned mineral mortar is extremely low and negligible in terms
to the manufacturing process. of health hazards. Options for applications in indoor
Powder residues: Residual product is returned to the areas with permanent stays by people: Evidence of the
production process wherever possible. emission performance of construction products in
Air: Process air is dedusted autonomously, whereby contact with indoor air and depending on the
the values are far below legal requirements. designated use must be submitted for applications in
Water: The production process does not involve water. indoor areas with permanent stays by people, e.g. in
Very low volumes of water are required for laboratory accordance with the German AgBB test scheme or the
tests and for sanitary facilities. GEV (Gemeinschaft Emissionskontrollierte
Noise: Noise level measurements have indicated that Verlegewerkstoffe, Klebstoffe und Bauprodukte e.V.,
all values established within the production facility fall Düsseldorf) EMICODE® marking system typically
below the hearing protection limit of 85dB(A). applied in Germany.
Waste: The main types of waste are powder waste,
paper (paper bags) and foil. Low volumes of metal 2.12 Reference service life
scrap (metal containers), waste oil (maintenance), Modified mineral mortars decisively improve the
wood (pallets) and commercial waste are incurred. All usability of building structures and significantly extend
waste is separated, stored and redirected to the their original service lives. The anticipated reference
recycling circuit or disposed of. service life depends on the specific installation
situation and the exposure associated with the product.
It can be influenced by weathering as well as
2.8 Product processing/Installation mechanical or chemical loads.
Modified mineral mortars can be processed both
automatically and manually. The mortars are either
automatically removed from a silo using a dry conveyor 2.13 Extraordinary effects
or manually taken from the container, mixed with water
and installed. The professional liability association's Fire
rules apply as well as the respective safety data sheets In accordance with Commission Decision 94/611EC,
pertaining to the construction products. On account of modified mineral binding agents comprising finely
the various hydrate levels of cement, lime and calcium distributed organic components must always be
sulphate binding agents in the mineral mortar, the classified in reaction-to-fire class A1 ‘No contribution to
fresh mortar mixed with water is usually strongly fire’ in accordance with EN 13501­1.
alkaline. In the case of more extensive contact, this Where higher percentages of organic components are
alkaline state can cause serious damage to eyes and involved, it can also be assumed that at least the
skin. Therefore, any contact with eyes or skin must be requirements of EN 13501­1 are maintained for fire
avoided by taking personal protective measures, and class E and Efl.
the information outlined on the safety data sheet must
be observed. Uncontrolled dust emissions should be
avoided. Modified mineral mortars may not be Fire protection
discharged into the sewage system, surface water or Name Value
groundwater. Waste incurred on the building site Building material class -
(packaging, pallets, residual mortar) must be collected Burning droplets -
separately. Suitable waste disposal companies Smoke gas development -
dispose of packaging materials and mortar sacks and
return them to the recycling circuit. Dry mortar residue Water
is taken back by the manufacturing plants and used as No relevant volumes of water-soluble substances
a raw material. No dry mortar residue in mortar sacks hazardous to water are washed out when hardened
is incurred. Hard mortar residue can be recycled or modified mineral mortars are exposed to water (e.g.
disposed of as building site rubble. flooding). Modified mineral mortar is stable in terms of
structure and is not subject to any changes in form
2.9 Packaging when exposed to water and drying. If non-hardened
A detailed description of packaging is provided in modified mineral mortars are exposed to water an
section 2.4. Empty, trickle-free paper containers and increase of the pH will take place.
clean PE foils can be recycled.
Mechanical destruction
The mechanical destruction of modified mineral
2.10 Condition of use mortars does not lead to any decomposition products
A modified mineral mortar does not rot and is resistant which are harmful to the environment or health. Dust
to ageing when used in accordance with the
5 Environmental Product Declaration DBC, EFCC, FEICA, IVK – Modified mineral mortar, group 2
incurred during de-construction should be avoided by amounts do not play a role when the construction
taking the appropriate measures (e.g. humidification). product is disposed of. They do not interfere with the
disposal/recycling of other components/building
materials.
2.14 Re-use phase The following waste codes according to the European
Components manufactured using modified mineral List of Waste (2000/532/EC) can apply:
mortars can usually be easily demolished. When a Mineral mortar: EWC 17 01 01 and EWC 10 13 14
building is removed, the materials do not need to be Mineral filler and levelling compound: EWC 17 01 07
treated as special waste; care should, however, be Calcium sulphate-based filler and levelling compound:
taken to ensure unmixed residual materials wherever EWC 17 08 02
possible. Modified mineral mortars can usually be
redirected to normal building material recycling circuits.
Re-use is generally in the form of recycled aggregate 2.16 Further information
in building construction and civil engineering. No More information is available on the manufacturer's
practical experience is currently available for reusing product or safety data sheets and is available on the
components comprising cementitious-based products manufacturer's websites or on request. Valuable
after decommissioning. technical information is also available on the
associations' websites.
2.15 Disposal
The portion of a modified mineral mortar applied to
another construction product is rather low. These low
3. LCA: Calculation rules
3.1 Declared Unit run the machines. After the demolition, the product is
This EPD refers to the declared unit of 1 kg of modified transported to the end-of-life processing (C2 module)
mineral mortar, group 2; applied into the building with a where all the impacts related to the transport
density of 800 - 1,700 kg/m³ in accordance with processes are considered. For precautionary principle
the IBU PCR part B for Mineral Factory-Made Mortars. and as a worst-case scenario, landfilling is the only
The results of the Life Cycle Assessment provided in end-of-life scenario considered. This is modelled by
this declaration have been selected from the product the landfill process (module C4) where the product
with the highest environmental impact (worst-case ends its life cycle.
scenario). Module D accounts for potential benefits that are
Depending on the application, a corresponding beyond the defined system boundaries. Credits are
conversion factor such as the density to convert generated during the incineration of packaging material
volumetric use to mass must be taken into that is occurring in the A5 module.
consideration.
The Declaration type is according to EN 15804: Cradle 3.3 Estimates and assumptions
to gate with options, modules C1–C4, and module D For this EPD formulation and production data defined
(A1–A3, C, D) and additional modules (A4-A5). and collected by FEICA were considered. Production
waste was assumed to be disposed of by landfilling as
Declared unit a worst-case.
Name Value Unit An average of paper sacks with polyethylene lining and
Declared unit 1 kg wooden pallets was considered in the LCA.
800 -
Gross density kg/m3
1700 3.4 Cut-off criteria
All raw materials submitted for the formulations and
production data were taken into consideration.
The manufacture of machinery, plant and other
3.2 System boundary infrastructure required for the production of the
Modules A1, A2 and A3 are taken into consideration in products under review was not taken into consideration
the LCA: in the LCA.
- A1 Production of preliminary products Transport of packaging materials is excluded.
- A2 Transport to the plant
- A3 Production incl. provision of energy, production of 3.5 Background data
packaging as well as auxiliaries and consumables and Data from the GaBi 10 database SP40 (2020) was
waste treatment used as background data.
- A4 Transport to site
- A5 Installation, product applied into the building 3.6 Data quality
during A5 phase operations and packaging disposal. Representative products were applied for this EPD and
The end of life for the packaging material considered is the product in the group displaying the highest
described below: environmental impact was selected for calculating the
-Incineration, for materials like plastic, wood and LCA results. The background datasets used are less
paper. than 4 years old.
-C1-C2-C4-D Production data and packaging are based on details
The building deconstruction (demolition process) takes provided by the manufacturer. The formulation used for
place in the C1 module which considers energy evaluation refers to a specific product.
generation and consumption of diesel and all the The data quality of the background data is considered
emissions connected with the fuel-burning process to to be good.
6 Environmental Product Declaration DBC, EFCC, FEICA, IVK – Modified mineral mortar, group 2
3.9 Comparability
3.7 Period under review Basically, a comparison or an evaluation of EPD data
Representative formulations are valid for 2021. is only possible if all the data sets to be compared
were created according to EN 15804 and the building
3.8 Allocation context, respectively the product-specific
Mass allocation has been applied when primary data characteristics of performance, are taken into account.
have been used and implemented into the LCA model.
The GaBi 10 database SP40 (2020) was used.
4. LCA: Scenarios and additional technical information
Characteristic product properties
Information on biogenic carbon
The packaging material contains biogenic carbon
content which is presented below.
Information on describing the biogenic Carbon
Content at factury gate
Name Value Unit
Biogenic Carbon Content in product - kg C
Biogenic Carbon Content in
0.0194 kg C
accompanying packaging
For the preparation of building life cycle assessments,
it must be taken into account that in module A5
(installation in the building) the biogenic amount of CO
2
(0.0194 kg C *3.67 = 0.071 kg CO -eq.) of the
2
packaging bound in module A1-A3 is mathematically
booked out.
Transport to the building site (A4)
Name Value Unit
Transport distance 1000 km
Gross weight 34 - 40 t
Payload capacity 27 t
Installation into the building (A5)
Name Value Unit
Other resources for packaging material 0.055 kg
Material loss 0.01 kg
Water consumption 0.0003 m3
Material loss considers the amount of product not used
during the application phase into the building. This
amount is 1 % of the product, impacts related to the
production of this part are accounted to the A5 module.
This percentage is considered as waste to disposal
and impacts of its end of life have been considered into
the LCA model and declared in A5.
End of life (C1-C4)
Name Value Unit
Collected as mixed construction waste 1.126 kg
Landfilling 1.126 kg
The value above 1 kg is due to the use of water during
the installation phase where 50 % of water evaporate
while 50 % remain in the product.
7 Environmental Product Declaration DBC, EFCC, FEICA, IVK – Modified mineral mortar, group 2
5. LCA: Results
DESCRIPTION OF THE SYSTEM BOUNDARY (X = INCLUDED IN LCA; ND = MODULE OR INDICATOR NOT
DECLARED; MNR = MODULE NOT RELEVANT)
BENEFITS AND
CONSTRUCTI LOADS
PRODUCT STAGE ON PROCESS USE STAGE END OF LIFE STAGE BEYOND THE
STAGE SYSTEM
BOUNDARIES
8 Environmental Product Declaration DBC, EFCC, FEICA, IVK – Modified mineral mortar, group 2
lairetam
waR
ylppus tropsnarT
gnirutcafunaM
eht
morf
tropsnarT
etis
eht
ot
etag
ylbmessA esU
ecnanetniaM
riapeR
tnemecalpeR tnemhsibrufeR
ygrene
lanoitarepO esu
retaw
lanoitarepO esu
noitcurtsnoc-eD
noitilomed tropsnarT
gnissecorp
etsaW
lasopsiD -esueR -yrevoceR -gnilcyceR laitnetop
A1 A2 A3 A4 A5 B1 B2 B3 B4 B5 B6 B7 C1 C2 C3 C4 D
X X X X X ND ND MNR MNR MNR ND ND X X ND X X
RESULTS OF THE LCA - ENVIRONMENTAL IMPACT according to EN 15804+A2: 1 kg of modified mineral
mortar, group 2
Core Indicator Unit A1-A3 A4 A5 C1 C2 C4 D
GWP-total [kg CO2-Eq.] 9.59E-1 5.06E-2 1.09E-1 3.14E-4 1.39E-2 1.72E-2 -3.50E-2
GWP-fossil [kg CO2-Eq.] 1.03E+0 5.00E-2 1.83E-2 3.00E-4 1.33E-2 1.71E-2 -3.49E-2
GWP-biogenic [kg CO2-Eq.] -6.90E-2 1.46E-4 9.10E-2 1.39E-5 6.10E-4 5.40E-5 -8.21E-5
GWP-luluc [kg CO2-Eq.] 8.48E-4 4.05E-4 1.01E-5 7.20E-9 3.14E-7 4.91E-5 -2.45E-5
ODP [kg CFC11-Eq.] 8.55E-12 6.01E-18 8.55E-14 3.19E-20 1.39E-18 6.33E-17 -3.66E-16
AP [mol H+-Eq.] 2.20E-3 1.50E-4 3.89E-5 4.06E-6 4.20E-5 1.22E-4 -4.90E-5
EP-freshwater [kg P-Eq.] 2.67E-6 1.52E-7 3.24E-8 6.47E-11 2.83E-9 2.93E-8 -4.52E-8
EP-marine [kg N-Eq.] 6.48E-4 6.68E-5 1.20E-5 1.84E-6 1.93E-5 3.15E-5 -1.27E-5
EP-terrestrial [mol N-Eq.] 7.12E-3 7.48E-4 1.48E-4 2.01E-5 2.13E-4 3.46E-4 -1.36E-4
POCP [kg NMVOC-Eq.] 2.17E-3 1.32E-4 3.66E-5 5.53E-6 3.81E-5 9.55E-5 -3.64E-5
ADPE [kg Sb-Eq.] 8.98E-8 3.59E-9 1.12E-9 9.07E-12 3.96E-10 1.53E-9 -5.74E-9
ADPF [MJ] 1.29E+1 6.66E-1 1.54E-1 4.29E-3 1.87E-1 2.24E-1 -5.92E-1
[m³ world-Eq
WDP 1.52E-1 4.47E-4 2.49E-2 5.93E-7 2.59E-5 1.79E-3 -3.63E-3
deprived]
GWP = Global warming potential; ODP = Depletion potential of the stratospheric ozone layer; AP = Acidification potential of land and water; EP =
Caption Eutrophication potential; POCP = Formation potential of tropospheric ozone photochemical oxidants; ADPE = Abiotic depletion potential for non-
fossil resources; ADPF = Abiotic depletion potential for fossil resources; WDP = Water (user) deprivation potential
RESULTS OF THE LCA - INDICATORS TO DESCRIBE RESOURCE USE according to EN 15804+A2: 1 kg of
modified mineral mortar, group 2
Indicator Unit A1-A3 A4 A5 C1 C2 C4 D
PERE [MJ] 1.91E+0 3.74E-2 7.52E-1 1.35E-5 5.90E-4 2.93E-2 -1.30E-1
PERM [MJ] 7.21E-1 0.00E+0 -7.21E-1 0.00E+0 0.00E+0 0.00E+0 0.00E+0
PERT [MJ] 2.63E+0 3.74E-2 3.08E-2 1.35E-5 5.90E-4 2.93E-2 -1.30E-1
PENRE [MJ] 1.17E+1 6.67E-1 2.30E-1 4.29E-3 1.87E-1 2.24E-1 -5.92E-1
PENRM [MJ] 1.17E+0 0.00E+0 -8.66E-2 0.00E+0 0.00E+0 0.00E+0 0.00E+0
PENRT [MJ] 1.29E+1 6.67E-1 1.43E-1 4.29E-3 1.87E-1 2.24E-1 -5.92E-1
SM [kg] 0.00E+0 0.00E+0 0.00E+0 0.00E+0 0.00E+0 0.00E+0 0.00E+0
RSF [MJ] 0.00E+0 0.00E+0 0.00E+0 0.00E+0 0.00E+0 0.00E+0 0.00E+0
NRSF [MJ] 0.00E+0 0.00E+0 0.00E+0 0.00E+0 0.00E+0 0.00E+0 0.00E+0
FW [m³] 4.16E-3 4.33E-5 5.88E-4 2.43E-8 1.06E-6 5.65E-5 -1.50E-4
PERE = Use of renewable primary energy excluding renewable primary energy resources used as raw materials; PERM = Use of
renewable primary energy resources used as raw materials; PERT = Total use of renewable primary energy resources; PENRE = Use of
non-renewable primary energy excluding non-renewable primary energy resources used as raw materials; PENRM = Use of non-
Caption
renewable primary energy resources used as raw materials; PENRT = Total use of non-renewable primary energy resources; SM = Use
of secondary material; RSF = Use of renewable secondary fuels; NRSF = Use of non-renewable secondary fuels; FW = Use of net fresh
water
RESULTS OF THE LCA – WASTE CATEGORIES AND OUTPUT FLOWS according to EN 15804+A2:
1 kg of modified mineral mortar, group 2
Indicator Unit A1-A3 A4 A5 C1 C2 C4 D
HWD [kg] 8.58E-5 3.10E-8 8.58E-7 4.16E-13 1.82E-11 3.42E-9 -2.36E-10
NHWD [kg] 6.53E-2 1.02E-4 1.47E-2 4.39E-7 1.92E-5 1.13E+0 -2.74E-4
RWD [kg] 4.10E-4 8.25E-7 5.38E-6 4.61E-9 2.01E-7 2.55E-6 -4.43E-5
CRU [kg] 0.00E+0 0.00E+0 0.00E+0 0.00E+0 0.00E+0 0.00E+0 0.00E+0
MFR [kg] 0.00E+0 0.00E+0 0.00E+0 0.00E+0 0.00E+0 0.00E+0 0.00E+0
MER [kg] 0.00E+0 0.00E+0 0.00E+0 0.00E+0 0.00E+0 0.00E+0 0.00E+0
EEE [MJ] 0.00E+0 0.00E+0 1.48E-1 0.00E+0 0.00E+0 0.00E+0 0.00E+0
EET [MJ] 0.00E+0 0.00E+0 2.66E-1 0.00E+0 0.00E+0 0.00E+0 0.00E+0
HWD = Hazardous waste disposed; NHWD = Non-hazardous waste disposed; RWD = Radioactive waste disposed; CRU = Components
Caption for re-use; MFR = Materials for recycling; MER = Materials for energy recovery; EEE = Exported electrical energy; EET = Exported
thermal energy
RESULTS OF THE LCA – additional impact categories according to EN 15804+A2-optional:
1 kg of modified mineral mortar, group 2
Indicator Unit A1-A3 A4 A5 C1 C2 C4 D
[Disease
PM ND ND ND ND ND ND ND
Incidence]
[kBq U235-
IRP ND ND ND ND ND ND ND
Eq.]
ETP-fw [CTUe] ND ND ND ND ND ND ND
HTP-c [CTUh] ND ND ND ND ND ND ND
HTP-nc [CTUh] ND ND ND ND ND ND ND
SQP [-] ND ND ND ND ND ND ND
PM = Potential incidence of disease due to PM emissions; IR = Potential Human exposure efficiency relative to U235; ETP-fw = Potential
Caption comparative Toxic Unit for ecosystems; HTP-c = Potential comparative Toxic Unit for humans (cancerogenic); HTP-nc = Potential
comparative Toxic Unit for humans (not cancerogenic); SQP = Potential soil quality index
Potential Human exposure efficiency relative to U235, Disclaimer 1 – This impact category deals mainly with the
eventual impact of low dose ionizing radiation on human health of the nuclear fuel cycle. It does not consider
effects due to possible nuclear accidents, occupational exposure or radioactive waste disposal in underground
facilities. Potential ionizing radiation from the soil, radon and (from) some construction materials is also not
measured by this indicator.
ADP minerals & metals, ADP fossil, WDP, ETF-fw, HTP-c, HTP-nc, SQP, Disclaimer 2 – The results of this
environmental impact indicator shall be used with care as the uncertainties on these results are high or as there is
limited experience with the indicator.
Additional environmental impact indicators (suggested by EN15804, table 4) are not declared in the EPD. The
results of this environmental impact indicator shall be used with care as the uncertainties on these results are high
and as there is limited experience with the indicator (see ILCD classification in EN 15804, table 5). For this
reason, results based on these indicators are not considered suitable for a decision-making process and are thus
not declared in the EPD.
6. LCA: Interpretation
The majority of impacts are associated with the In all EPDs, CO is the most important contributor to
2
production phase (A1-A3). The most significant Global Warming Potential (GWP). For the Acidification
contribution to the production phase impacts is the Potential (AP), NOx and SO contribute the largest
2
upstream production of raw materials as the main share.
driver. Besides the cement also the dispersion powder Transportation to the construction site (A4) and the
influences the results significantly, although this is only installation process (A5) make a minor contribution to
used for up to 9 % of the total composition. Significant almost all impacts. The only exception is a relevant
contributions to Primary Energy Demand – Non- influence of carbon dioxide emissions in module A5 to
renewable (PENRT) derive from the energy resources Global Warming Potential (GWP) due to the
used in the production of raw materials. The largest incineration of the packaging materials plastic, paper
contributor to Primary Energy Demand – Renewable and pallets.
(PERT) is the consumption of renewable energy In module A4, transport to construction site, values for
resources required for the generation and supply of Eutrophication (freshwater, marine and terrestrial)
electricity. During manufacturing (A1-A3) some have an impact due principally to the emission of
influence also arises due to the wooden pallets and phosphate. Furthermore, climate change from land use
paper used as packaging that need solar energy for change is influenced by transport processes, due to
photosynthesis. It should be noted that Primary Energy the diesel production used as fuel, because part of this
Demand – Renewable (PERT) generally represents a diesel has been produced from bio-based raw
small percentage of the production phase primary materials.
energy demand with the bulk of the demand coming The end-of-life phases have a negligible influence on
from non-renewable energy resources. all impacts.
7. Requisite evidence
Leaching If of relevance for the application (usually if the
Special tests and evidence have not been carried out products are used outside of buildings) the leaching
or provided within the framework of drawing up this behaviour has to be measured e.g. according to DIN
Model EPD. Some member states require special EN 12457/1­­4 or DIN EN 14405 combined with the
documentation on leaching for specific areas of Council decision 2003/33/EC.
application. This documentation has to be provided
separately and is specific to the product in question.
8. References
EN 998-1
9 Environmental Product Declaration DBC, EFCC, FEICA, IVK – Modified mineral mortar, group 2
EN 998-1:2016, Specification for mortar for masonry – particle size below 10 mm (without or with limited size
Part 1: Rendering and plastering mortar reduction)
EN 1015-17 EN 13279
EN 1015-17:2005-01, Methods of test for mortar for EN 13279-1:2008, Gypsum binders and gypsum
masonry – Part 17: Determination of water-soluble plasters – Part 1: Definitions and requirements
chloride content of fresh mortars
EN 13501-1
EN 1504-3 EN 13501-1:2018, Fire classification of construction
EN 1504-3:2005-12, Products and systems for the products and building products – Part 1: Classification
protection and repair of concrete structures – using data from reaction to fire tests
Definitions, requirements, quality control and
evaluation of conformity – Part 3: Structural and non- EN 13813
structural repair EN 13813:2002-10, Screed material and floor screeds
– Screed materials – Properties and requirements
EN 1504-7
EN 1504-7:2006-08, Products and systems for the EN 13888
protection and repair of concrete structures – EN 13888:2009, Grout for tiles – Requirements,
Definitions, requirements, quality control and evaluation of conformity, classification and designation
evaluation of conformity – Part 7: Reinforcement
corrosion protection EN 13892-8
EN 13892-8:2003-02, Methods of test for screed
EN 1542 materials – Part 8: Determination of bond strength
EN 1542:1999-07, Products and systems for the
protection and repair of concrete structures – Test ISO 14025
methods – Measurement of bond strength by pull-off DIN EN ISO 14025:2011-10, Environmental labels and
declarations — Type III environmental declarations —
EN 12004 Principles and procedures
EN 12004:2012, Adhesives for tiles – Requirements,
evaluation of conformity, classification and designation DIN EN 14405
DIN EN 14405:2017-05, Characterization of waste -
EN 12004-2 Leaching behaviour test - Up-flow percolation test
EN 12004-2:2017, Adhesives for ceramic tiles - Part 2: (under specified conditions)
Test methods
EN 14891
EN 12190 EN 14891:2012-04, Liquid-applied water impermeable
EN 12190:1998-12, Products and systems for the products for use beneath ceramic tiling bonded with
protection and repair of concrete structures – Test adhesives – Requirements, test methods, evaluation of
methods – Determination of compressive strength of conformity, classification and designation
repair mortar
EN 15183
DIN EN 12457-1 EN 15183:2006-11, Products and systems for the
DIN EN 12457-1:2003-01, Characterization of waste - protection and repair of concrete structures – Test
Leaching; Compliance test for leaching of granular and methods – Corrosion protection test
sludges - Part 1: One stage batch test at a liquid to
solid ration of 2 l/kg with particle size below 4 mm EN 15804
(without or with size reduction) EN 15804+A2+AC:2021, Sustainability of construction
works — Environmental Product Declarations — Core
DIN EN 12457-2 rules for the product category of construction products
DIN EN 12457-2:2003-01, Characterization of waste -
Leaching; Compliance test for leaching of granular and EAD 030295-00-0605
sludges - Part 2: One stage batch test at a liquid to EAD 030295-00-0605, Flexible polymer modified
solid ratio of 10 l/kg with particle size below 4 mm mineral thick coating
(without or with size reduction)
EAD 030352-00-0503
EAD 030352-00-0503:2019:01, Liquid applied
DIN EN 12457-3 watertight covering kits for wet room floors and/or walls
DIN EN 12457-3:2021-03, Characterization of waste -
Leaching - Compliance test for leaching of granular EAD 040083-00-0404
waste materials and sludges - Part 3: Two stage batch EAD 040083-00-0404:2013, External Thermal
test at a liquid to solid ratio of 2 l/kg and 8 l/kg for Insulation Composite Systems with Rendering
materials with high solid content with particle size
below 4 mm (without or with size reduction) 96/603/EC
Commission decision of 4 October 1996 for specifying
a directory of products to be classified as category A
DIN EN 12457-4 "No contribution to fire" in accordance with decision
DIN EN 12457-4:2003-01, Characterization of waste - 94/611/EC on construction products for implementing
Leaching; Compliance test for leaching of granular Article 20 of Directive 89/106/EEC
waste materials and sludges - Part 4: One stage batch
test at a liquid to solid ratio of 10 l/kg for materials with 2000/532/EC
10 Environmental Product Declaration DBC, EFCC, FEICA, IVK – Modified mineral mortar, group 2
Commission decision dated 3 May 2000 replacing GaBi 10: Software and database for comprehensive
decision 94/3/EC on a waste directory in accordance analysis. LBP, University of Stuttgart and Sphera, 2020
with Article 1 a) of Council Directive 75/442/EEC on
waste and Council decision 94/904/EC on a directory GaBi 10 documentation
of hazardous waste in terms of Article 1, paragraph 4 Gabi 10: documentation of GaBi 10 data sets from the
of Directive 91/689/EEC on hazardous waste data base for Life Cycle Engineering LBP, University of
Stuttgart and Sphera, http://documentation.gabi-
2003/33/EC: software.com/, 2020
Council Decision of 19 December 2002 establishing
criteria and procedures for the acceptance of waste at IBU 2021
landfills pursuant to Article 16 of and Annex II to Institut Bauen und Umwelt e.V.: General Instructions
Directive 1999/31/EC for the EPD programme of Institut Bauen und Umwelt
e.V. EPD programme. Version 2.0. Berlin: Institut
Candidate list Bauen und Umwelt e.V., 2021
Candidate List of substances of very high concern for www.ibu-epd.com
Authorisation, published in accordance with Article
59(10) of the REACH Regulation, ECHA, MVV TB
www.echa.europa.eu/candidate-list-table Ü-mark in accordance with ‘Model Administrative
Order laying down Technical Building Regulations’
CPR (MVV TB) no. C 2.1.4.5
CPR Regulation (EU) No 305/2011 of the European
Parliament and of the Council of 9 March 2011 laying PCR Part A
down harmonised conditions for the marketing of Product Category Rules for Building-Related Products
construction products and repealing Council Directive and Services, Part A: Calculation Rules for the Life
89/106/EEC Cycle Assessment and Requirements on the Project
report, Version 1.1, Institut Bauen und Umwelt e.V.,
DAfStb Guideline 2021-01
DAfStb Guideline on ‘Production and use of cement-
bound flow concrete and grouting mortar’ (VeBMR), PCR Part B
2019-07 Product Category Rules for Construction Products,
Part B: Mineral Factory-Made Mortars, 2017-11
Decopaint Directive
Directive 2004/42/CE of the European Parliament and PG AIV
the council of 21 April 2004 on the limitation of Testing principles regarding the issuing of general
emissions of volatile organic compounds due to the building authority test certificates for waterproofing with
use of organic solvents in certain paints and varnishes waterproofing in conjunction with ceramic tiles (PG-
and vehicle refinishing products and amending AIV:2018-03)
Directive 1999/13/EC
PG MDS/FPD
EWC 101314 Testing principles regarding the issuing of general
2000/532/EC European Waste Catalogue / Ordinance building authority test certificates for waterproofing with
on European List of Wastes: Waste concrete and mineral waterproofing slurries and flexible polymer
concrete sludge thick coatings (PG-MDS/FPD:2016-11)
EWC 170101 REACH
2000/532/EC European Waste Catalogue / Ordinance Directive (EG) No. 1907/2006 of the European
on European List of Wastes: Concrete Parliament and of the Council dated 18 December
2006 on the registration, evaluation, approval and
EWC 170107 restriction of chemical substances (REACH), for
2000/532/EC European Waste Catalogue / Ordinance establishing a European Agency for chemical
on European List of Wastes: Mixtures of concrete, substances, for amending Directive 1999/45/EC and
bricks, tiles and ceramics for annulment of Directive (EEC) No. 793/93 of the
Council, Directive (EC) No. 1488/94 of the
EWC 170802 Commission, Guideline 76/769/EEC of the Council and
2000/532/EC European Waste Catalogue / Ordinance Guidelines 91/155/EEC, 93/67/EEC, 93/105/EC and
on European List of Wastes: Gypsum based 2000/21/EC of the Commission.
construction metals e.g. for plasterboard
GaBi 10
11 Environmental Product Declaration DBC, EFCC, FEICA, IVK – Modified mineral mortar, group 2
Publisher
Institut Bauen und Umwelt e.V. Tel +49 (0)30 3087748- 0
Hegelplatz 1 Fax +49 (0)30 3087748- 29
10117 Berlin Mail info@ibu-epd.com
Germany Web www.ibu-epd.com
Programme holder
Institut Bauen und Umwelt e.V. Tel +49 (0)30 - 3087748- 0
Hegelplatz 1 Fax +49 (0)30 – 3087748 - 29
10117 Berlin Mail info@ibu-epd.com
Germany Web www.ibu-epd.com
Author of the Life Cycle
Assessment Tel +49 711 341817-0
Sphera Solutions GmbH Fax +49 711 341817-25
Hauptstraße 111- 113 Mail info@sphera.com
70771 Leinfelden-Echterdingen Web www.sphera.com
Germany
Owner of the Declaration
FEICA - Association of the Tel +32 (0)267 673 20
European Adhesive and Sealant Fax +32 (0)267 673 99
Industry Mail info@feica.eu
Rue Belliard 40 box 10 Web www.feica.eu
1040 Brussels
Belgium
Tel +32289720-39
Fax +32289720-37
EFCC - European Federation for Mail info@efcc.be
Construction Chemicals Web www.efcc.eu
Boulevard du Triomphe 172
1160 Brussels
Belgium
Tel +49 (0)69 2556-1318
Fax +49 (0)69 2556-1319
Mail info@deutsche-bauchemie.de
Deutsche Bauchemie e.V. Web www.deutsche-bauchemie.de
Mainzer Landstr. 55
60329 Frankfurt
Germany
Tel +49 (0)211 67931-10
Fax +49 (0)211 67931-33
Mail info@klebstoffe.com
Industrieverband Klebstoffe e.V Web www.klebstoffe.com
Völklinger Straße 4
40219 Düsseldorf
Germany
