ENVIRONMENTAL PRODUCT DECLARATION
as per ISO 14025 and EN 15804+A2
Owner of the Declaration dormakaba International Holding GmbH
Publisher Institut Bauen und Umwelt e.V. (IBU)
Programme holder Institut Bauen und Umwelt e.V. (IBU)
Declaration number EPD-DOR-20230249-CBA1-EN
Issue date 30.06.2023
Valid to 29.06.2028
MTL Hybrid Lock Series
dormakaba
www.ibu-epd.com | https://epd-online.com
General Information
dormakaba MTL Hybrid Lock Series
Programme holder Owner of the declaration
IBU – Institut Bauen und Umwelt e.V. dormakaba International Holding GmbH
Hegelplatz 1 DORMA Platz 1
10117 Berlin 58256 Ennepetal
Germany Germany
Declaration number Declared product / declared unit
EPD-DOR-20230249-CBA1-EN 1 piece of the product: MTL Hybrid Lock Series, consisting of the following
items:
• MTL 9291/MTL 9291-II hybrid lock
• BLE digital hookbolt lockcase
• Forend
• Product packaging
This declaration is based on the product category rules: Scope:
Building Hardware products, 01.08.2021 This Environmental Product Declaration refers to a specific hybrid lock
(PCR checked and approved by the SVR) manufactured by dormakaba. Parts of the products are produced in China
and the final assembly takes place in Eskilstuna (Sweden).
Issue date The data represents the year 2022.
30.06.2023
The owner of the declaration shall be liable for the underlying information
and evidence; the IBU shall not be liable with respect to manufacturer
information, life cycle assessment data and evidences.
Valid to
29.06.2028 The EPD was created according to the specifications of EN 15804+A2. In
the following, the standard will be simplified as EN 15804.
Verification
The standard EN 15804 serves as the core PCR
Independent verification of the declaration and data according to ISO
14025:2011
internally X externally
Dipl.-Ing. Hans Peters
(Chairman of Institut Bauen und Umwelt e.V.)
Florian Pronold Matthias Klingler,
(Managing Director Institut Bauen und Umwelt e.V.) (Independent verifier)
1 Environmental Product Declaration - dormakaba - MTL Hybrid Lock Series
Product
Product description/Product definition Base materials/Ancillary materials
The MTL 9291/MTL 9291-II is a battery-powered hybrid lock The major material composition including packaging of the
that communicates via Bluetooth Low Energy (BLE). The lock is product is listed below:
opened via a smartphone (Android/Apple operating system). All Name Value Unit
electronics are integrated inside the lock case and no visible
Steel 57 %
devices need to be mounted on the outside of the door leaf.
Zinc 9 %
The lock also functions fully mechanically with the cylinder and
door handle. Plastic 31 %
For the use and application of the product the respective Electronics 2 %
national provisions at the place of use apply. For the MTL Batteries 2 %
Hybrid Lock Series the standards which can be applied are the
following:
The product includes partial articles which contain substances
• EN 14846
listed in the Candidate List of REACH Regulation
• EN 1634-1
1907/2006/EC (date: 17.01.2023) exceeding 0.1 percentage by
• SSF 3522 rev.2 class 3
mass: no
• SSF 3523 rev.1 class S3
The Candidate List can be found on the ECHA website:
The CE marking takes into account the proof of conformity with
https://echa.europa.eu/de/home.
the respective harmonized standards based on the legal
provisions above. Reference service life
The reference service life of the MTL Hybrid Lock Series is
Application
about 10 years, depending on the application and frequency of
The MTL Hybrid Lock Series is the ideal application to grant
use. For repairs and renewals, suitable spare parts are
controlled access to multiple users. Temporary access is also
available. The hybrid locks are tested and certified to EN
possible. It can be controlled via an app or Bluetooth Low
14846, meaning they are designed to withstand a minimum of
Energy (BLE).
200.000 cycles.
Technical Data
The MTL Hybrid Lock Series has following technical properties:
Name Value Unit
Category of use High Use 3 Grade
Test
Durability 200000
cycles
Load on latch bolt 120 N
Door mass and closing force 200 MTL 9291 = 9
Grade
kg, 15N MTL 9291-II = 6
MTL 9291 = C
Fire/smoke doors 30 minutes Grade
MTL 9291-II = F
Safety no requirement 0 Grade
Corrosion High resistance L Grade
Security and drill resistance Very
7 Grade
high
Protective effect of the electrical
1 Grade
functions EN 14846:2008
Proective effect of the electrical
3 Grade
manipulation EN 14846:2008
The products are not harmonised in accordance with the
Construction Product Regulations (CPR) but in accordance with
other provisions for harmonisation of the EU. Compliance with
the European Union Directive and technical specifications:
• Directive (EU) No 2011/65 (RoHS)
• Regulation (EC) No 1907/2006 (REACH)
• EN 14846
• EN 1634-1
• SSF 3522 rev.2 class 3
• SSF 3523 rev.1 class S3
The products are subject to CE marking according to the
relevant harmonization legislation.
2 Environmental Product Declaration - dormakaba - MTL Hybrid Lock Series
LCA: Calculation rules
Maintenance – Module B2
Declared Unit This module includes the production and the end of life of the
The declared unit is 1 piece of the product: MTL Hybrid Lock batteries. The potential use of batteries is declared in module
including packaging B2.
Name Value Unit
Declared unit 1 piece/product End-of-life stage– Modules C1-C4 and D
The end-of-life stage includes:
Mass of declared Product 1 kg
— C1, de-construction, demolition:
— C2, transport to waste processing;
— C3, waste processing for reuse, recovery and/or recycling;
System boundary
— C4, disposal;
The type of EPD is: cradle to gate with options, modules C1–
including provision and all transport, provision of all materials,
C4, and module D (A1–A3 + C + D and additional modules: A4
products and related energy and water use.
+ A5 + B2)
Module D (Benefits and loads beyond the system boundary)
Production - Modules A1-A3
includes:
The product stage includes:
— D, recycling potentials, expressed as net impacts and
— A1, raw material extraction, processing and mechanical
benefits.
treatments, processing of secondary material input (e.g.
recycling processes), Geographic Representativeness
— A2, transport to the manufacturer, Land or region, in which the declared product system is
— A3, manufacturing and assembly including provision of all manufactured, used or handled at the end of the product´s
materials, products and energy, as well as waste processing up lifespan: Europe
to the end-of waste state.
Construction stage - Modules A4-A5 Comparability
The construction process stage includes: Basically, a comparison or an evaluation of EPD data is only
— A4, transport to the building site; possible if all the data sets to be compared were created
— A5, installation into the building; including provision of all according to EN 15804 and the building context, respectively
materials, products and energy, as well as waste processing up the product-specific characteristics of performance, are taken
to the end-of waste state or disposal of final residues during the into account. Background database: GaBi, SP40.
construction process stage.
LCA: Scenarios and additional technical information
Maintenance (B2)
Characteristic product properties of biogenic carbon
Name Value Unit
Information on describing the biogenic carbon content at
Use of batteries 5 pieces
factory gate
Name ValueUnit dormakaba hybrid locks are operated using a battery and are
not connected to mains electricity. The battery is provided by
kg
Biogenic carbon content in product - dormakaba. During the operation of the product, the only
C
energy consumption comes from the battery use. The battery
Biogenic carbon content in accompanying kg
- must be changed on average 5 times over the declared service
packaging C
life. In order to allow scaling, the exchange of 1 battery is
declared in the LCA.
Transport to the building site (A4) Reference service life
Name Value Unit Name Value Unit
Litres of fuel 0.00276 l/100km Life Span according to the manufacturer 10 a
Transport distance 100 km
End of life (C1-C4)
Capacity utilisation (including empty runs) 55 %
C1: The product dismantling from the building is done
The product is transported via truck. The product is stored in manually without environmental burden.
the dormakaba plant in Eskilstuna (Sweden). The main C2: Transport to waste management 50 km.
distribution regions are Scandinavia and the Baltic States. In
Name Value Unit
order to allow scaling to a specific point of installation 100 km
Collected separately waste type waste type 0.73 kg
are declared.
Recycling 0.68 kg
Energy recovery 0.04 kg
Installation into the building (A5)
Landfilling 0.02 kg
Name Value Unit
Waste packaging 0,27 kg
3 Environmental Product Declaration - dormakaba - MTL Hybrid Lock Series
The product is disassembled in a recycling process. Material
recycling is then assumed for the metals and electronics. The
plastic components are assumed to be incinerated with energy
recovery. The batteries and minor proportions of residues
arising from the recycling process are landfilled. Region for the
End of LIfe is: Europe.
Reuse, recovery and/or recycling potentials (D), relevant
scenario information
Name Value Unit
Recycling 100 %
The collection rate is 100%.
4 Environmental Product Declaration - dormakaba - MTL Hybrid Lock Series
LCA: Results
DESCRIPTION OF THE SYSTEM BOUNDARY (X = INCLUDED IN LCA; ND = MODULE OR INDICATOR NOT DECLARED; MNR =
MODULE NOT RELEVANT)
Benefits and
Construction loads beyond
Product stage Use stage End-of-life stage
process stage the system
boundaries
la ire ta m w a Ry lp p u s tro p s n a rT g n iru tc a fu n a M e h t m o rf tro p s n a rTe tis e h t o t e ta g y lb m e s s A e s U e c n a n e tn ia M ria p e R tn e m e c a lp e R tn e m h s ib ru fe R y g re n e la n o ita re p Oe s u re ta w la n o ita re p Oe s u n o itc u rts n o c -e Dn o itilo m e d tro p s n a rT g n is s e c o rp e ts a W la s o p s iD -e s u e R-y re v o c e R-g n ilc y c e Rla itn e to p
A1 A2 A3 A4 A5 B1 B2 B3 B4 B5 B6 B7 C1 C2 C3 C4 D
X X X X X MND X MNR MNR MNR MND MND X X X X X
RESULTS OF THE LCA - ENVIRONMENTAL IMPACT according to EN 15804+A2: 1 piece MTL Hybrid Lock Series
Parameter Unit A1-A3 A4 A5 B2 C1 C2 C3 C4 D
GWP-total kg CO 2 eq 6.32E+00 9E-03 6.86E-01 2.61E-01 0 3E-03 9.5E-02 2.73E-04 -1.72E+00
GWP-fossil kg CO 2 eq 6.27E+00 8E-03 6.86E-01 2.6E-01 0 3E-03 9.5E-02 2.72E-04 -1.72E+00
GWP-biogenic kg CO 2 eq 4.3E-02 3.87E-04 1.6E-05 4.82E-04 0 1.47E-04 2.2E-06 9.28E-07 3E-03
GWP-luluc kg CO 2 eq 6.86E-03 2E-07 3.88E-05 2.5E-04 0 7.55E-08 5.35E-06 7.82E-07 -2E-03
ODP kg CFC11 eq 2.12E-10 8.85E-19 3.46E-16 4.91E-12 0 3.35E-19 4.77E-17 1.01E-18 -6.39E-15
AP mol H+ eq 3.3E-02 8.39E-06 1.22E-04 8.14E-04 0 3.17E-06 1.68E-05 1.95E-06 -7E-03
EP-freshwater kg P eq 1.68E-05 1.79E-09 5.52E-08 4.18E-07 0 6.79E-10 7.61E-09 4.66E-10 -2.14E-06
EP-marine kg N eq 6.35E-03 2.67E-06 2.76E-05 1.79E-04 0 1.01E-06 3.8E-06 5.01E-07 -1E-03
EP-terrestrial mol N eq 6.5E-02 2.97E-05 5.57E-04 2.01E-03 0 1.12E-05 7.67E-05 5.51E-06 -1.1E-02
kg NMVOC
POCP 1.8E-02 7.55E-06 7.62E-05 4.9E-04 0 2.86E-06 1.05E-05 1.52E-06 -3E-03
eq
ADPE kg Sb eq 1.02E-03 2.51E-10 4.75E-09 1.14E-06 0 9.51E-11 6.54E-10 2.44E-11 -1.77E-04
ADPF MJ 9.15E+01 1.19E-01 3.18E-01 3.36E+00 0 4.5E-02 4.4E-02 4E-03 -2.26E+01
m3 world eq
WDP 1.23E+00 1.64E-05 7E-02 3.5E-02 0 6.21E-06 1E-02 2.85E-05 -4.76E-01
deprived
GWP = Global warming potential; ODP = Depletion potential of the stratospheric ozone layer; AP = Acidification potential of land and water; EP =
Eutrophication potential; POCP = Formation potential of tropospheric ozone photochemical oxidants; ADPE = Abiotic depletion potential for non-fossil
resources; ADPF = Abiotic depletion potential for fossil resources; WDP = Water (user) deprivation potential)
RESULTS OF THE LCA - INDICATORS TO DESCRIBE RESOURCE USE according to EN 15804+A2: 1 piece MTL Hybrid Lock
Series
Parameter Unit A1-A3 A4 A5 B2 C1 C2 C3 C4 D
PERE MJ 1.34E+01 3.75E-04 8.3E-02 6.75E-01 0 1.42E-04 1.1E-02 4.67E-04 -4.3E+00
PERM MJ 0 0 0 0 0 0 0 0 0
PERT MJ 1.34E+01 3.75E-04 8.3E-02 6.75E-01 0 1.42E-04 1.1E-02 4.67E-04 -4.3E+00
PENRE MJ 7.82E+01 1.19E-01 1.19E+01 3.36E+00 0 4.5E-02 1.78E+00 4E-03 -2.27E+01
PENRM MJ 1.33E+01 0 -1.16E+01 0 0 0 -1.73E+00 0 0
PENRT MJ 9.15E+01 1.19E-01 3.18E-01 3.36E+00 0 4.5E-02 4.4E-02 4E-03 -2.27E+01
SM kg 4.09E-01 0 0 0 0 0 0 0 0
RSF MJ 0 0 0 0 0 0 0 0 0
NRSF MJ 0 0 0 0 0 0 0 0 0
FW m3 4.21E-02 6.72E-07 2E-03 2E-03 0 2.54E-07 2.31E-04 8.99E-07 -1.8E-02
PERE = Use of renewable primary energy excluding renewable primary energy resources used as raw materials; PERM = Use of renewable primary
energy resources used as raw materials; PERT = Total use of renewable primary energy resources; PENRE = Use of non-renewable primary energy
excluding non-renewable primary energy resources used as raw materials; PENRM = Use of non-renewable primary energy resources used as raw
materials; PENRT = Total use of non-renewable primary energy resources; SM = Use of secondary material; RSF = Use of renewable secondary fuels;
NRSF = Use of non-renewable secondary fuels; FW = Use of net fresh water
RESULTS OF THE LCA – WASTE CATEGORIES AND OUTPUT FLOWS according to EN 15804+A2:
1 piece MTL Hybrid Lock Series
Parameter Unit A1-A3 A4 A5 B2 C1 C2 C3 C4 D
HWD kg 1.79E-06 1.15E-11 1.21E-09 4.21E-08 0 4.37E-12 1.67E-10 5.43E-11 -1.88E-07
NHWD kg 2.77E-01 1.22E-05 7.1E-02 6.4E-02 0 4.6E-06 1E-02 1.8E-02 -7.5E-02
RWD kg 1.5E-03 1.28E-07 1.18E-05 7.8E-05 0 4.83E-08 1.63E-06 4.06E-08 -6.61E-04
CRU kg 0 0 0 0 0 0 0 0 0
MFR kg 0 0 0 0 0 0 7.04E-01 0 0
MER kg 0 0 0 0 0 0 0 0 0
EEE MJ 6.86E-05 0 1.27E+00 0 0 0 0 0 0
EET MJ 1.25E-04 0 2.92E+00 0 0 0 0 0 0
5 Environmental Product Declaration - dormakaba - MTL Hybrid Lock Series
HWD = Hazardous waste disposed; NHWD = Non-hazardous waste disposed; RWD = Radioactive waste disposed; CRU = Components for re-use;
MFR = Materials for recycling; MER = Materials for energy recovery; EEE = Exported electrical energy; EET = Exported thermal energy
RESULTS OF THE LCA – additional impact categories according to EN 15804+A2-optional:
1 piece MTL Hybrid Lock Series
Parameter Unit A1-A3 A4 A5 B2 C1 C2 C3 C4 D
Disease
PM 3.88E-07 4.41E-11 1.56E-09 8.54E-09 0 1.67E-11 2.15E-10 2.41E-11 -1.13E-07
incidence
IR kBq U235 eq 2.01E-01 1.83E-05 1E-03 8E-03 0 6.9E-06 1.47E-04 4.17E-06 -9.5E-02
ETP-fw CTUe 5.25E+01 8.4E-02 1.19E-01 1.15E+01 0 3.2E-02 1.6E-02 2E-03 -9.06E+00
HTP-c CTUh 2.94E-07 1.59E-12 1.03E-11 5.82E-11 0 6E-13 1.42E-12 3.02E-13 -9E-10
HTP-nc CTUh 1.28E-07 6.78E-11 1.05E-09 6.74E-09 0 2.56E-11 1.44E-10 3.32E-11 1.29E-07
SQP SQP 1.07E+01 3.05E-04 9.5E-02 3.28E-01 0 1.16E-04 1.3E-02 7.43E-04 -2.76E+00
PM = Potential incidence of disease due to PM emissions; IR = Potential Human exposure efficiency relative to U235; ETP-fw = Potential comparative
Toxic Unit for ecosystems; HTP-c = Potential comparative Toxic Unit for humans (cancerogenic); HTP-nc = Potential comparative Toxic Unit for humans
(not cancerogenic); SQP = Potential soil quality index
Disclaimer 1 – for the indicator “Potential Human exposure efficiency relative to U235”. This impact category deals mainly with the
eventual impact of low-dose ionizing radiation on human health of the nuclear fuel cycle. It does not consider effects due to possible
nuclear accidents, occupational exposure or radioactive waste disposal in underground facilities. Potential ionizing radiation from the
soil, radon and from some construction materials is also not measured by this indicator.
Disclaimer 2 – for the indicators “abiotic depletion potential for non-fossil resources”, “abiotic depletion potential for fossil resources”,
“water (user) deprivation potential, deprivation-weighted water consumption”, “potential comparative toxic unit for ecosystems”,
“potential comparative toxic unit for humans – cancerogenic”, “Potential comparative toxic unit for humans - not cancerogenic”,
“potential soil quality index”. The results of this environmental impact indicator shall be used with care as the uncertainties on these
results are high as there is limited experience with the indicator.
This EPD was created using a software tool.
References
ISO 14025
DIN EN ISO 14025:2011-10, Environmental labels and Further References
declarations — Type III environmental declarations —
Principles and procedures IBU 2021
General Instructions for the EPD programme of Institut Bauen
EN 14846 und Umwelt e.V. Version 2.0, Berlin: Institut
EN 14846:2018 Bauen und Umwelt e.V., 2021. www.ibu-epd.com
Building hardware - Locks and latches - Electromechanically
operated locks and striking plates - Requirements and test GaBi
methods Sphera Solutions GmbH
Gabi Software System and Database for Life Cycle Engineering
EN 15804 19922020
EN 15804+A2:2019+AC:2021, Version 10.0.0.71
Sustainability University of Stuttgart
of construction works — Environmental Product Declarations — Leinfelden-Echterdingen
Core rules for the product category of construction products
GaBi ts documentation
EN 1634-1 GaBi life cycle inventory data documentation (https://www.gabi-
EN 1634-1:2014+A1:2018; software.com/support/gabi/gabidatabase- 2020-lci-
Fire resistance and smoke control tests for door and shutter documentation/).
assemblies, openable windows and elements of building
hardware LCA-tool dormakaba
LCA tool, version DHW.
SSF 3522 Tool No.: IBU-DOR-202104-LT1-EN.
SSF 3522:2018 Developed by Sphera Solutions GmbH
Burglar resistant fixed mounted lock units
PCR Part A
SSF 3523 PCR – Part A: Calculation Rules for the Life Cycle Assessment
SST 3523:2020 and Requirements on the Project Re-port according to EN
Digital locking unit 15804+A2:2019, Version 1.0, 2020, Institut Bauen und Umwelt
e.V., www.ibu-epd.com.
REACH
Regulation (EC) No 1907/2006 of the European PCR Part B
Parliament and of the Council on the Registration, PCR – Part B: Requirements on the EPD for Building Hardware
Evaluation, Authorisation and Restriction of Chemicals product, version 1.2, Institut Bauen und Umwelt e.V., www.ibu-
(REACH) epd.com, 2017.
6 Environmental Product Declaration - dormakaba - MTL Hybrid Lock Series
Publisher
Institut Bauen und Umwelt e.V. +49 (0)30 3087748- 0
Hegelplatz 1 info@ibu-epd.com
10117 Berlin www.ibu-epd.com
Germany
Programme holder
Institut Bauen und Umwelt e.V. +49 (0)30 3087748- 0
Hegelplatz 1 info@ibu-epd.com
10117 Berlin www.ibu-epd.com
Germany
Author of the Life Cycle Assessment
dormakaba International Holding GmbH +49 2333 793-0
DORMA Platz 1 info.de@dormakaba.com
58256 Ennepetal www.dormakaba.com
Germany
Owner of the Declaration
dormakaba International Holding GmbH +49 2333 793-0
DORMA Platz 1 info.de@dormakaba.com
58256 Ennepetal www.dormakaba.com
Germany
7 Environmental Product Declaration - dormakaba - MTL Hybrid Lock Series
