ENVIRONMENTAL PRODUCT DECLARATION
as per ISO 14025 and EN 15804+A2
Owner of the Declaration NedZink B.V.
Programme holder Institut Bauen und Umwelt e.V. (IBU)
Publisher Institut Bauen und Umwelt e.V. (IBU)
Declaration number EPD-NED-20200256-IBA1-EN
Issue date 22.03.2022
Valid to 21.03.2027
NedZink NATUREL
NedZink B.V.
www.ibu-epd.com | https://epd-online.com
Umwelt Produktdeklaration Name des Herstellers – Name des Produkts
1. General Information
NedZink B.V. NedZink NATUREL
Programme holder Owner of the declaration
IBU – Institut Bauen und Umwelt e.V. NedZink B.V.
Panoramastr. 1 Hoofdstraat 1
10178 Berlin 6024 AA, Budel-Dorplein
Germany Netherlands
Declaration number Declared product / declared unit
EPD-NED-20200256-IBA1-EN 1kg NedZink® NATUREL, bright-rolled titanium zinc
This declaration is based on the product Scope:
category rules: The Life Cycle Assessment (LCA) was carried out
Building metals, 11.2017 according to ISO 14040, ISO 14044 and EN 15804.
(PCR checked and approved by the SVR) The LCA is performed for NedZink® NATUREL
manufactured by NedZink B.V. in Budel-Dorplein,
Netherlands.
Issue date
The natural rolled zinc from NedZink covered by this
22.03.2022
EPD can be used in buildings as roof, façade or
rainwater systems.
Valid to The LCA was carried out for the manufacturing phase
21.03.2027 of the declared product, containing information on raw
and secondary material production, transport and
packaging (cradle to gate). Possible credits after the
end of life phase (module D), demolition (C1), transport
to waste processing and disposal (C2), waste
processing (C3) and waste disposal (C4) are also
included.
The owner of the declaration shall be liable for the
underlying information and evidence; the IBU shall not
be liable with respect to manufacturer information, life
cycle assessment data and evidences.
The EPD was created according to the specifications
of EN 15804+A2. In the following, the standard will be
simplified as EN 15804.
Verification
The standard EN 15804 serves as the core PCR
Independent verification of the declaration and data
according to ISO 14025:2010
Dipl. Ing. Hans Peters internally x externally
(chairman of Institut Bauen und Umwelt e.V.)
Dr. Alexander Röder Mr Olivier Muller
(Managing Director Institut Bauen und Umwelt e.V.)) (Independent verifier)
2. Product
2.1 Product description/Product definition the quality management system at NedZink assure a
NedZink® NATUREL is titanium zinc produced by constant and uniform high-quality standard.
NedZink according to EN 988.
Small quantities, as specified in EN 988, of the alloy For the placing on the market of the product in the
elements copper, titanium and aluminium are added to European Union/European Free Trade Association
electrolytically refined zinc (with a purity of min. (EU/EFTA) (with the exception of Switzerland)
99,995% Zn, Z1 according to EN 1179). Regulation (EU) No. 305/2011 (CPR) applies. The
The chemical composition, mechanical and physical product needs a Declaration of Performance taking
properties and measurement tolerances are into consideration EN 14782:2006, Self-supporting
determined in the KOMO product certificate and metal sheet for roofing, external cladding and internal
certified as NedZink NTZ® by Lloyd's Register Product lining, or EN 14783:2013, Fully supported metal sheet
certificate (approval No QIS 122). and strip for roofing, external cladding and internal
The defined material properties are checked by an lining, and the CE-marking.
independent and neutral research institute. This For the application and use the respective national
product certification and the ISO 9001 certificate for provisions apply.
2 Environmental Product Declaration NedZink B.V. – NedZink Naturel
Concern for Authorisation (SVHC) dated 01/2018. The
2.2 Application product does not contain substances with carcinogenic
NedZink® NATUREL titanium zinc coils, sheets, strips mutagenic reprotoxic (CMR) properties >0.1%.
and profiles are used for:
- roof and façade cladding (CE-marked based on This product/article/at least one partial article contains
EN14782:2006, Self-supporting metal sheet substances listed in the candidate list (dated 01/2018)
for roofing, external cladding and internal lining exceeding 0.1 percentage by mass: no
or EN14783:2013, Fully supported metal sheet and
strip for roofing, external cladding and internal lining) This product/article/at least one partial article contains
- interior use other CMR substances in categories 1A or 1B which
- roof drainage systems (gutters, downpipes and are not on the candidate list, exceeding 0.1 percentage
accessories according to EN612) by mass: no
- ornaments
Biocide products were added to this construction
2.3 Technical Data product or it has been treated with biocide products
The main constructional data are presented in the (this then concerns a treated product as defined by the
following table: (EU) Ordinance on Biocide Products No. 528/2012):
no
Constructional data
Name Value Unit
Coefficient of thermal expansion 22 10-6K-1 2.6 Manufacture
Tensile strength ≥ 150 N/mm2 The manufacturing process of high grade rolled zinc
Not includes the following steps:
Compressive strength N/mm2
relevant
Modulus of elasticity ≥ 80000 N/mm2 Pre-alloy:
Melting point 420 °C In order to improve the properties of zinc, and for
Thermal conductivity 110 W/(mK) energy saving purposes, a pre-alloy with titanium,
Electrical conductivity at 20°C 17000000 Ω-1m-1 copper and aluminium is prepared in an induction
furnace. This pre-alloy is poured into ingots.
Density 7200 kg/m3
Required testing standards are described in EN 988.
Melting:
In the melting furnace the Special High Grade (SHG)
Performance data of the product in accordance with
zinc and the ingots are mixed homogeneously. Zinc
the declaration of performance with respect to its
with the right composition is pumped to the casting
essential characteristics according to EN
furnace.
14782 and EN 14783 respectively.
Casting:
2.4 Delivery status
Casting takes place from the casting furnace into a
NedZink material is delivered in thicknesses from 0.5
vertical casting installation. The zinc is cast into blocks,
to 1.5 mm. As average production data is considered,
cooled down with a closed water system and stored for
the LCIA results reflect the environmental profile of
further processing.
weighted average product thickness: 0.727 mm.
The maximum width of sheets, coils and strips is 1000
Rolling and coiling:
mm.
Blocks coming from the casting installation are
The standard sheets are delivered in 1000 x 2000 mm,
homogeneous pre-heated for the “hot rolling” process.
1000 x 2250 mm and 1000 x 3000 mm.
This takes place in a gas-fired continuous oven.
Finished products are delivered to customer
During the hot rolling on a reversible rolling machine
specification.
the blocks are processed to a predefined thickness. At
the end of the rolling installation the zinc is coiled and
Application rules:
stored to cool off.
EN988:1996, Zinc and zinc alloys - Specifications for
On the reversible cold-rolling mill the coils are rolled to
rolled flat products for buildings
the desired final thickness. For cooling and lubrication
EN612:2005, Eaves gutters with bead stiffened fronts
of the process a special emulsion is used
and rainwater pipes with seamed joints made of metal
sheet
Stretching and cutting:
Tension in the coils is released by a stretching- and
2.5 Base materials/Ancillary materials
straightening process. The zinc is uniquely marked and
Components of NedZink alloy
slitted and cut to the desired width and length.
The composition of bright rolled zinc from NedZink is in
accordance with EN988:
Quality control:
- Special-High-Grade zinc 99.995% (Z1 according to
During the entire process extensive quality checks are
EN 1179)
conducted by the manufacturer and Lloyd's Register.
- Copper: 0.08 - 0.17%
Quality Management according to ISO 9001.
- Titanium: 0.07 - 0.12%
Product quality is checked by Lloyd's Register and
- Aluminium: ≤ 0.015%
approved with an Industrial Quality Scheme Approval
Certificate QIS122.
Auxiliary substances
Lubricant oil: 0.65 kg/t zinc.
Additionally, the quality control is audited by Kiwa and
certified with KOMO product certificates:
None of the components included in the final product is
- BRL2034, KOMO K7054/04 zinc sheets
listed in the Candidate List of Substances of Very High
3 Environmental Product Declaration NedZink B.V. – NedZink Naturel
- BRL2035, KOMO K7057/04 zinc gutters The material has a repellent effect to electrosmog
- BRL2044, KOMO K7063/04 zinc downpipes (electromagnetic radiation) and the effects of rain and
snow may be neglected.
2.7 Environment and health during
manufacturing 2.11 Environment and health during use
The manufacturing process is carried out according to Environment
the rules as laid down in the environmental permit. The due to air and water formed patina (zinc
NedZink’s policy follows the Total Quality Management carbonate) is a natural protection layer. Due to this
(TQM). patina the transfer of zinc ions via rain water is
The directives of the Environmental Management constantly reduced, because this protection layer is
System ISO14001 are an integral part of the Quality non-water-soluble.
Management System ISO9001. Further transfer of zinc ions is mainly related to the air
pollution with SO . Due to the reduction of SO
2 2
2.8 Product processing/Installation concentration in the air, the zinc-concentration of
Basic principles: precipitation in the rainwater has subsequently been
NedZink material must be stored under dry and reduced to one fifth of the former values during the last
ventilated conditions. This applies to storage in thirty years.
warehouses, on building sites, on installation sites as As a result of all environmental regulations this amount
well as during transportation. Coils are to be stored on will reduce even more in the future, due to the
their original pallets. reduction of SO concentration in the air. The transfer
2
of zinc ions via rain water is constantly reduced due to
Transportation should only be done in the development of a natural protection layer of zinc
enclosed vehicles. carbonate.
Temperature deviations have to be avoided as it can In aquatic systems only a small part of the total zinc
result in varying humidity levels. concentration is available for organisms (bioavailable).
All contact between zinc and moisture (wet surface, It is related to the physical-chemical conditions of the
rain or dew) during handling and transportation must receiving water body.
be avoided. Wet surfaces (with or without protective
film) may not directly be covered. Health
When used according to their designated function,
The material is to be processed without tension. NedZink products will have no health effects.
Zinc is an essential metal, necessary for living
The thermal expansion has to be taken into account organisms. Zinc does not accumulate in the body.
when installing/handling the product. The recommended daily intake of zinc (in the correct
form) according to the WHO is 15mg/day for men
Mechanical deformation of zinc should be avoided in and12mg/day for women.
case the zinc temperature is not at least 7°C.
2.12 Reference service life
Further installation rules are listed on The service life depends on the correct application
www.nedzink.com. according to the guidelines for processing and
installation. The theoretical lifetime according to the
2.9 Packaging available literature is > 100 years.
The packaging material in use are wooden pallets, Service lifetime according to Bundesinstitut für Bau-
paper/cardboard and plastics (films and wires). All Stadt- und Raumforschung (BBSR): > 50 years.
packaging materials are reusable and/or recyclable, if
gathered separately. As the EPD scope is a cradle-to-gate with options, no
The take-back and recycling of our packaging in reference service life is declared in the LCA.
Germany is organized by Interseroh.
The standard ISO 15686 has not been considered.
2.10 Condition of use 2.13 Extraordinary effects
NedZink material develops a protective patina layer,
which darkens the material slightly over time due to a Fire
reaction with oxygen and carbon dioxide (air and The NedZink® products comply with EN13501-1: the
water). This layer is responsible for the high resistance requirements of building material Class A1 "non-
of titanium zinc against corrosion. combustible". (96/603/EC)
Zinc in contact with air creates a zinc-oxide. Due to the
influence of water a zinc-hydroxide is developed. In the Fire protection
final step a reaction with carbon dioxide creates a non- Name Value
water-soluble coating of basic zinc carbonate, being Building material class EN13501 DIN4102 A1
the patina. Therefore NedZink material does not Burning droplets EN13501 D0
require any maintenance and cleaning during the Smoke gas development EN13501 -
period of use. If the surface is slightly damaged, this
naturally formed patina layer will heal itself. Smoke production
Vaporization as zinc oxide (ZnO) occurs when heated
NedZink material is UV-resistant, non-flammable and above 650 °C. The produced ZnO smoke may cause
resistant to radiating heat. Direct contact with chemical zinc fever (diarrhoea, dry throat, feverish) when
substances, especially those containing acids, has to inhaled over some (period of) time. The effects
be avoided. A list of substances to be avoided can be disappear completely in 1 to 2 days after the
found on www.nedzink.com.
4 Environmental Product Declaration NedZink B.V. – NedZink Naturel
inhalation. which is no longer valuable for the internal production
process, is completely recycled by a third party
Water (European Waste Code 10.05.01).
Zinc is not classified as hazardous for the aquatic
environment. The scrap from demolition and renovation work on
building sites is collected and sold either directly to
Mechanical destruction secondary smelting works or via a scrap metal dealer.
Given the metallic nature of the product, there will be The recycling rate for zinc sheets is over 95%. Credits
no environmental effect. for this recycling are appointed in module D. These
credits are based on a recycling percentage of 95%
2.14 Re-use phase (European recycling rate for rolled zinc).
Disassembly:
During disassembly of a building construction or 2.15 Disposal
renovations, NedZink material should be separated Due to the effective recycling process, a maximum of
from other materials. Zinc can then easily be collected 5% zinc has to be disposed.
for re-use and/or recycling. The European Waste Code for collected zinc after
disassembly is 17.04.04.
Re-use/Recycling:
Scrap produced during the manufacturing process 2.16 Further information
from NedZink material are 100% remelted and fed Additional information, optional details, references,
back completely into NedZink's production process. A data sheets can be obtained at: www.nedzink.com
small amount of residue (skimmings, dross, dust),
3. LCA: Calculation rules
3.1 Declared Unit The environmental impact of the SHG Zinc was then
The declared unit is 1 kg of NedZink NATUREL, bright- calculated using SimaPro V9.0. Site-specific data was
rolled titanium zinc. provided by NedZink and verified against earlier
studies.
Declared unit
Name Value Unit 3.6 Data quality
Declared unit 1 kg The data used for this study was both of high quality
conversion factor [Mass/Declared and recent. The specific data was collected by the
1 -
Unit] manufacturer, The generic data that is used is less
Gross density 7200 kg/m3 than 10 years old or has been updated within this
period. This is in compliance with the data quality
requirements of EN 15804.
3.2 System boundary 3.7 Period under review
Type of the EPD: Cradle-to-Gate with options. Modules Site-specific data for the years 2019 and 2020 was
A1, A2 and A3 contain information on the raw- and used in this study. Background data is taken from the
secondary material extraction, transport to the Ecoinvent V3.6 database (2019) and varies in age.
manufacturer, manufacturing and packaging.
Module C1 - C4 (end of life) and module D (applicable 3.8 Allocation
to the aforementioned modules) are declared. Modules Allocation was avoided in this study, as required in EN
A4, A5 and B1-B7 are not declared. 15804. However, in the background database,
allocation can be applied.
3.3 Estimates and assumptions
No major assumptions and estimations were 3.9 Comparability
necessary for the LCA. Basically, a comparison or an evaluation of EPD data
is only possible if all the data sets to be compared
3.4 Cut-off criteria were created according to EN 15804 and the building
No major cut-offs were applied to specific context, respectively the product-specific
manufacturing data from Nedzink. Production impacts characteristics of performance, are taken into account.
of packaging for raw materials are not known and
excluded, waste processing of this packaging is known The used background database is Ecoinvent
and included. For upstream data a background V3.6 database (2019).
database (Ecoinvent V3.6) was used, which can
contain additional cut-offs.
3.5 Background data
Background processes are taken from the Ecoinvent
V3.6 database (2019), with the “allocation, cut-off by
classification” system model.
Life cycle inventory data for the production of zinc
concentrate and SHG Zinc in the Ecoinvent
V3.6 database is updated with the most recent LCA
report (Zinc Environmental Profile - 2015 Update) on
primary Zinc by the International Zinc Association
(IZA).
5 Environmental Product Declaration NedZink B.V. – NedZink Naturel
4. LCA: Scenarios and additional technical information
Characteristic product properties
Information on biogenic Carbon
The biogenic carbon content quantifies the amount of
biogenic carbon in a construction product leaving the
factory gate, and it shall be separately declared for the
product and for any accompanying packaging. If the
total mass of biogenic carbon-containing materials is
less than 5 % of the total mass of the product and
accompanying packaging, the declaration of biogenic
carbon content may be omitted. The mass of
packaging containing biogenic carbon shall always be
declared. Note: 1 kg biogenic Carbon is equivalent to
44/12 kg of CO2
Modules A4, A5, B1-B7 are not considered in this
study. The possible credits given in Module D are
based on 100% recyclability of zinc products. After the
collection (a collection rate of 95% is taken), zinc scrap
is re-melted and converted to secondary zinc. This is
not done by NedZink but by third parties. The possible
credit for the zinc gained through re-melting is
calculated using the dataset of the primary zinc
production. The remaining zinc (5%) is landfilled
(module C4).
End of life (C4) / Recycling potentials (D)
Name Value Unit
Recycling 95% kg
Landfilling 5% kg
6 Environmental Product Declaration NedZink B.V. – NedZink Naturel
5. LCA: Results
Disclaimer:
EP-freshwater: This indicator has been calculated as “kg P eq” as required in the characterization model
(EUTREND model, Struijs et al., 2009b, as implemented in ReCiPe;
http://eplca.jrc.ec.europa.eu/LCDN/developerEF.xhtml)
DESCRIPTION OF THE SYSTEM BOUNDARY (X = INCLUDED IN LCA; ND = MODULE OR INDICATOR NOT
DECLARED; MNR = MODULE NOT RELEVANT)
BENEFITS AND
CONSTRUCTI LOADS
PRODUCT STAGE ON PROCESS USE STAGE END OF LIFE STAGE BEYOND THE
STAGE SYSTEM
BOUNDARIES
7 Environmental Product Declaration NedZink B.V. – NedZink Naturel
lairetam
waR
ylppus tropsnarT
gnirutcafunaM
eht
morf
tropsnarT
etis
eht
ot
etag
ylbmessA esU
ecnanetniaM
riapeR
tnemecalpeR tnemhsibrufeR
ygrene
lanoitarepO esu
retaw
lanoitarepO esu
noitcurtsnoc-eD
noitilomed tropsnarT
gnissecorp
etsaW
lasopsiD -esueR -yrevoceR -gnilcyceR laitnetop
A1 A2 A3 A4 A5 B1 B2 B3 B4 B5 B6 B7 C1 C2 C3 C4 D
X X X ND ND ND ND MNR MNR MNR ND ND X X X X X
RESULTS OF THE LCA - ENVIRONMENTAL IMPACT according to EN 15804+A2: 1 kg of NEDZINK natural
Core Indicator Unit A1-A3 C1 C2 C3 C4 D
Global warming potential - total [kg CO2-Eq.] 3.22E+0 1.73E-4 6.92E-3 5.73E-2 2.64E-4 -2.50E+0
Global warming potential - fossil fuels [kg CO2-Eq.] 3.11E+0 1.73E-4 6.91E-3 5.72E-2 2.63E-4 -2.39E+0
Global warming potential - biogenic [kg CO2-Eq.] 9.82E-2 4.82E-8 4.20E-6 3.09E-5 5.22E-7 -1.04E-1
GWP from land use and land use change [kg CO2-Eq.] 9.86E-3 1.37E-8 2.45E-6 9.83E-6 7.34E-8 -8.17E-3
Depletion potential of the stratospheric ozone layer [kg CFC11-Eq.] 2.46E-7 3.74E-11 1.59E-9 1.19E-8 1.08E-10 -1.77E-7
Acidification potential, accumulated exceedance [mol H+-Eq.] 2.85E-2 1.81E-6 3.94E-5 5.84E-4 2.50E-6 -2.36E-2
Eutrophication, fraction of nutrients reaching freshwater
end compartment
[kg PO4-Eq.] 3.26E-4 6.31E-10 5.69E-8 3.48E-7 2.95E-9 -2.81E-4
Eutrophication, fraction of nutrients reaching marine end
[kg N-Eq.] 6.10E-3 8.01E-7 1.41E-5 2.54E-4 8.60E-7 -5.08E-3
compartment
Eutrophication, accumulated exceedance [mol N-Eq.] 6.89E-2 8.78E-6 1.55E-4 2.79E-3 9.48E-6 -5.73E-2
Formation potential of tropospheric ozone photochemical
[kg NMVOC-Eq.] 1.75E-2 2.42E-6 4.44E-5 7.67E-4 2.75E-6 -1.43E-2
oxidants
Abiotic depletion potential for non-fossil resources [kg Sb-Eq.] 6.78E-2 2.66E-10 1.79E-7 9.37E-8 2.41E-9 -6.30E-2
Abiotic depletion potential for fossil resources [MJ] 4.54E+1 2.39E-3 1.06E-1 7.85E-1 7.36E-3 -3.55E+1
Water (user) deprivation potential, deprivation-weighted [m³ world-Eq
2.81E+0 3.20E-6 3.26E-4 1.43E-3 3.30E-4 -2.59E+0
water consumption (WDP) deprived]
RESULTS OF THE LCA - INDICATORS TO DESCRIBE RESOURCE USE according to EN 15804+A2: 1 kg of
NEDZINK natural
Indicator Unit A1-A3 C1 C2 C3 C4 D
Renewable primary energy as energy carrier [MJ] 6.10E+0 1.29E-5 1.52E-3 8.27E-3 5.95E-5 -4.83E+0
Renewable primary energy resources as material utilization [MJ] 2.64E-1 0.00E+0 0.00E+0 0.00E+0 0.00E+0 0.00E+0
Total use of renewable primary energy resources [MJ] 6.37E+0 1.29E-5 1.52E-3 8.27E-3 5.95E-5 -4.83E+0
Non-renewable primary energy as energy carrier [MJ] 4.84E+1 2.53E-3 1.13E-1 8.34E-1 7.82E-3 -3.78E+1
Non-renewable primary energy as material utilization [MJ] 0.00E+0 0.00E+0 0.00E+0 0.00E+0 0.00E+0 0.00E+0
Total use of non-renewable primary energy resources [MJ] 4.84E+1 2.53E-3 1.13E-1 8.34E-1 7.82E-3 -3.78E+1
Use of secondary material [kg] 1.33E-1 0.00E+0 0.00E+0 0.00E+0 0.00E+0 8.15E-1
Use of renewable secondary fuels [MJ] 0.00E+0 0.00E+0 0.00E+0 0.00E+0 0.00E+0 0.00E+0
Use of non-renewable secondary fuels [MJ] 0.00E+0 0.00E+0 0.00E+0 0.00E+0 0.00E+0 0.00E+0
Use of net fresh water [m³] 8.64E-2 1.23E-7 1.20E-5 5.87E-5 7.86E-6 -7.70E-2
RESULTS OF THE LCA – WASTE CATEGORIES AND OUTPUT FLOWS according to EN 15804+A2:
1 kg of NEDZINK natural
Indicator Unit A1-A3 C1 C2 C3 C4 D
Hazardous waste disposed [kg] 8.63E-3 6.50E-9 2.71E-7 2.06E-6 1.10E-8 -8.14E-3
Non-hazardous waste disposed [kg] 4.40E-1 2.83E-6 6.57E-3 1.06E-3 5.00E-2 -3.51E-1
Radioactive waste disposed [kg] 2.19E-4 1.66E-8 7.21E-7 5.32E-6 4.83E-8 -1.84E-4
Components for re-use [kg] 0.00E+0 0.00E+0 0.00E+0 0.00E+0 0.00E+0 0.00E+0
Materials for recycling [kg] 0.00E+0 0.00E+0 0.00E+0 9.50E-1 0.00E+0 0.00E+0
Materials for energy recovery [kg] 0.00E+0 0.00E+0 0.00E+0 0.00E+0 0.00E+0 0.00E+0
Exported electrical energy [MJ] 0.00E+0 0.00E+0 0.00E+0 0.00E+0 0.00E+0 0.00E+0
Exported thermal energy [MJ] 0.00E+0 0.00E+0 0.00E+0 0.00E+0 0.00E+0 0.00E+0
RESULTS OF THE LCA – additional impact categories according to EN 15804+A2-optional:
1 kg of NEDZINK natural
Indicator Unit A1-A3 C1 C2 C3 C4 D
Potential incidence of disease due to PM emissions [Disease
1.16E-7 4.80E-11 6.24E-10 1.52E-8 4.85E-11 -8.07E-8
Incidence]
Potential Human exposure efficiency relative to U235 [kBq U235-
3.00E-1 1.02E-5 4.64E-4 3.37E-3 3.02E-5 -2.65E-1
Eq.]
Potential comparative toxic unit for ecosystems [CTUe] 6.20E+2 1.44E-3 8.61E-2 5.04E-1 4.77E-3 -5.69E+2
Potential comparative toxic unit for humans - cancerogenic [CTUh] 1.52E-8 5.03E-14 3.07E-12 1.68E-11 1.10E-13 -1.40E-8
Potential comparative toxic unit for humans - not cancerogenic [CTUh] 4.55E-7 1.24E-12 1.03E-10 4.19E-10 3.41E-12 -4.13E-7
Potential soil quality index [-] 2.36E+1 3.05E-4 9.07E-2 1.16E-1 1.54E-2 -1.83E+1
Disclaimer 1 – for the indicator IRP:
This impact category deals mainly with the eventual impact of low dose ionizing radiation on human health of the
nuclear fuel cycle. It does not consider effects due to possible nuclear accidents, occupational exposure nor (due
to) radioactive waste disposal in underground facilities. Potential ionizing radiation from the soil, from radon and
(from) some construction materials is also not measured by this indicator.
Disclaimer 2 – for the indicators ADPE, ADPF, WDP, ETP-fw, HTP-c, HTP-nc, SQP:
The results of this environmental impact indicator shall be used with care as the uncertainties on these results are
high or as there is limited experience with the indicator.
6. LCA: Interpretation
The main impact categories for 1 kg of Nedzink The remaining contributions mainly consist of energy
NATUREL usage (electricity and gas) with a small contribution
from the remaining metal components (Cu, Ti, Al).
Life cycle inventory data for the production of zinc
concentrate and Special High-Grade Zinc (SHG Zinc) Because of the high contribution of SHG Zinc and the
in the background database Ecoinvent V3.6 is aligned high recyclability that is assumed, the amount of
with data from the IZA 2015 LCA report (Zinc credits gained in module D for each impact category is
Environmental Profile - 2015 Update, see also section very high, at least 75% or higher compared to the initial
3.5 Background Data). impact value.
The contribution of SHG Zinc is the dominating factor
in all of the impact categories, with contributions >80%
in for all indicators.
7. Requisite evidence
In a literature study TNO-MEP-99/441 of TNO (Dutch lower than the corrosion rate. The growth of the patina
Organisation for Applied Scientific Research) the layer delays the corrosion.
emissions from corrosion of zinc to water have been The run-off rate is influenced by the atmospheric
evaluated. This corrosion rate refers to the loss of conditions, of which the SO concentration is the most
2
metallic zinc. important variable. With the decreasing of the SO
2
The run-off rate is the wash-off of zinc from the patina concentration, the corrosion rate is also decreasing.
layer. This run-off rate is generally lower than the
corrosion rate. In areas with higher SO -concentration a run-off rate of
2
3 g/m2.yr can be calculated and 2 g/m2.yr in areas with
During the built-up of the zinc patina layer the run-off is lower concentration.
8 Environmental Product Declaration NedZink B.V. – NedZink Naturel
8. References
General Programme Instructions
Institut Bauen und Umwelt e.V., Berlin (pub.): The EN 15804
preparation of environmental product declarations EN 15804:2012+A2:2019
(EPDs); General Programme Instructions for the Sustainability of construction works - Environmental
preparation of EPDs at the Institut Bauen und Umwelt Product Declarations - Core rules for the product
e.V. (IBU) V2.0, 2021 category of construction products
www.ibu-epd.com
DIN 4102
PCR 2021 Part A DIN 4102
Institut Bauen und Umwelt e.V., Berlin: Product Fire behaviour of building materials and building
Category Rules for Construction Products from the components
range of Environmental Product Declarations of Institut
Bauen und Umwelt (IBU), Part A: Calculation Rules for ISO 9001
the Life Cycle Assessment and Requirements on the ISO 9001:2015
Background Report according to EN 15804+A2:2019. Quality management systems - Requirements
Version 1.1, January 2021
www.ibu-epd.com ISO 14001
ISO 14001:2015
PCR 2017 Part B Environmental management systems - Requirements
Institut Bauen und Umwelt e.V., Berlin: Product with guidance for use
Category Rules for Construction Products from the
range of Environmental Product Declarations of Institut ISO 14025
Bauen und Umwelt (IBU), Part B: Requirements on the ISO 14025:2011-10
EPD for Building Metals. Version 1.6, November 2017 Environmental labels and declarations - Type III
www.ibu-epd.com environmental declarations - Principles and procedures
EN 612 ISO 14040
EN 612:2005 ISO 14040:2006
Eaves gutters with bead stiffened fronts and rainwater Environmental management - Life cycle assessment -
pipes with seamed joints made of metal sheet Principles and framework
EN 988 ISO 14044
EN 988:1996 ISO 14044:2006
Zinc and zinc alloys - Specification for rolled flat Environmental management - Life cycle assessment -
products for building Requirements and guidelines
EN 1179 ISO 15686
EN 1179:2003 ISO 15686
Zinc and zinc alloys - Primary zinc Buildings and constructed assets - Service life
planning
EN 13501-1
EN 13501-1:2007+A1:2009 Regulation (EU) No. 305/2011
Fire classification of construction products and building Regulation (EU) No 305/2011 of the European
elements - Part 1: Classification using data from Parliament and of the Council of 9 March 2011 laying
reaction to fire tests down harmonised conditions for the marketing of
construction products and repealing Council Directive
EN 13501-5 89/106/EEC (Text with EEA relevance)
EN 13501-5:2006+A1:2009
Fire classification of construction products and building 96/603/EC
elements - Part 5: Classification using data from EU Commission Decision of 4 October 1996
external fire exposure to roofs tests establishing the list of products belonging to Classes A
'No contribution to fire' provided for in Decision
EN 14782 94/611/EC implementing Article 20 of Council Directive
EN 14782:2006 89/106/EEC on construction products (Text with EEA
Self-supporting metal sheet for roofing, external relevance)
cladding and internal lining - Product specification and
requirements KOMO product certificates
BRL2034: K7054/04 zinc sheets
EN 14783 BRL2035: K7057/04 zinc gutters
EN 14783:2013 BRL2044: K7063/04 zinc downpipes
Fully supported metal sheet and strip for roofing,
external cladding and internal lining - Product Lloyd's Register Product certificate (approval No
specification and requirements QIS 122)
Lloyd’s Register Inspection Services - Product
certificate Industrial Quality Scheme for Product
9 Environmental Product Declaration NedZink B.V. – NedZink Naturel
Certification by Surveillance of Quality Systems
(approval No QIS 122) Zinc…A Sustainable Material
International Zinc Association (2010)
Candidate List of substances of very high concern
for Authorisation Zinc, A Sustainable Material – Essential for Modern
ECHA published in accordance with Article 59(10) of Life.
the REACH Regulation (2018) International Zinc Association (2017)
Bundesinstitut für Bau-, Stadt- und International Zinc Association (IZA)
Raumforschung (BBSR) Global industry association dedicated to the interests
Nutzungsdauer von Bauteilen für of zinc and its users
Lebenszyklusanalysen nach BNB (BNB: www.zinc.org
Bewertungssystem Nachhaltiges Bauen)(2011)
SimaPro V9.0
TNO-MEP-99/441 Life Cycle Assessment software
Diffusive Emissions of zinc due to atmospheric
corrosion of zinc and zinc-coated (galvanised) Ecoinvent V3.6
materials - R.H.J. Korenromp, J.C.Th. Hollander Life Cycle Inventory database, 2019
(1999)
Zinc Environmental Profile - 2015 Update
International Zinc Association (2016)
Zinc Recycling, Closing the Loop
International Zinc Association (2011)
10 Environmental Product Declaration NedZink B.V. – NedZink Naturel
Publisher
Institut Bauen und Umwelt e.V. Tel +49 (0)30 3087748- 0
Panoramastr. 1 Fax +49 (0)30 3087748- 29
10178 Berlin Mail info@ibu-epd.com
Germany Web www.ibu-epd.com
Programme holder
Institut Bauen und Umwelt e.V. Tel +49 (0)30 - 3087748- 0
Panoramastr 1 Fax +49 (0)30 – 3087748 - 29
10178 Berlin Mail info@ibu-epd.com
Germany Web www.ibu-epd.com
Author of the Life Cycle
Assessment Tel +31 (0)30-693 00 55
Stichting Adviescentrum Metaal Fax +31 (0)30-693 00 57
Kelvinbaan 40 Mail info@metaaladvies.nl
3430MT Nieuwegein Web metaaladvies.nl
Netherlands
Owner of the Declaration
NedZink B.V. Tel +31 (0)475 455700
Hoofdstraat 1 Fax +31 (0)475 455790
6024AA Budel-Dorplein Mail info@nedzink.com
Netherlands Web www.nedzink.com
