ENVIRONMENTAL PRODUCT DECLARATION
as per ISO 14025 and EN 15804+A2
Owner of the Declaration Rubner Holding AG - S.p.A.
Publisher Institut Bauen und Umwelt e.V. (IBU)
Programme holder Institut Bauen und Umwelt e.V. (IBU)
Declaration number EPD-NOR-20230235-IBD2-EN
Issue date 28.06.2023
Valid to 27.06.2028
Nordpan – Solid wood panels (Update)
Nordpan GmbH - Srl
www.ibu-epd.com | https://epd-online.com
1. General Information
Nordpan GmbH - Srl Nordpan – Solid wood panels (Update)
Programme holder Owner of the declaration
IBU – Institut Bauen und Umwelt e.V. Rubner Holding AG - S.p.A.
Hegelplatz 1 Handwerkerzone 2
10117 Berlin 39030 Kiens
Germany Italy
Declaration number Declared product / declared unit
EPD-NOR-20230235-IBD2-EN 1 m³ of NORDPAN solid wood panels with an average density of 493 kg/m³
This declaration is based on the product category rules: Scope:
Solid wood products, 01.08.2021 This EPD is based on a declared unit of 1 m³ of NORDPAN solid wood
(PCR checked and approved by the SVR) panels (moisture of 9 % at a raw density of 493 kg/m³). The results refer to
a representative average of one- to five-layered nordpan solid wood
panels. The LCA covers 100 % of nordpan's production referring to its sites
Issue date located at Strassen (Austria) and Olang (Italy).
28.06.2023
The owner of the declaration shall be liable for the underlying information
and evidence; the IBU shall not be liable with respect to manufacturer
information, life cycle assessment data and evidences.
Valid to
27.06.2028 The EPD was created according to the specifications of EN 15804+A2. In
the following, the standard will be simplified as EN 15804.
Verification
The standard EN 15804 serves as the core PCR
Independent verification of the declaration and data according to ISO
14025:2011
internally X externally
Dipl.-Ing. Hans Peters
(Chairman of Institut Bauen und Umwelt e.V.)
Florian Pronold Matthias Schulz,
(Managing Director Institut Bauen und Umwelt e.V.) (Independent verifier)
1 Environmental Product Declaration - Nordpan GmbH - Srl - Nordpan – Solid wood panels (Update)
2. Product
Constructional data
2.1 Product description/Product definition
NORDPAN solid wood panel (NORDPAN-SWP) is a Name Value Unit
homogenized wood-based plate-like material that is used in Wood types by trade names acc. spruce, pine, larch,
-
engineered structural timber constructions, façade construction, to EN 1912 Douglas fir
decorative interior design as well as for doors and furniture. Wood moisture acc. to EN
< 15 %
NORDPAN-SWP consists of one to five layers made from kiln- 13183-1
dried coniferous wood laminations which are glued together at
Use of wood preservatives (the Where other
their wide faces orthogonally. Due to the bonded cross-
wood preservative test mark to preservative means -
sectional structure combined with the technically supported
/DIN 68800-3/ must be indicated) are insufficient
strength and stiffness classification of the raw materials,
Bending strength (out of plane)
NORDPAN-SWP is characterized by a high product quality. As 12 to 35 N/mm²
acc. to EN 13353
a result of the industrial manufacturing process, NORDPAN-
SWP exhibits steady mechanical characteristics. Planar Bending strength (in plane) acc. 10 to 25 N/mm²
NORDPAN-SWP shows a high dimensional stability and can be to EN 13353
characterized as a largely crack-minimized building material. Modulus of elasticity (in plane)
1800 to 4700 N/mm²
For the placing on the market of the product in the European acc. to EN 13353
Union/European Free Trade Association (EU/EFTA) (with the Modulus of elasticity (out of
550 to 10000 N/mm²
exception of Switzerland) Regulation (EU) No. 305/2011 /CPR plane) acc. to EN 13353
applies. The product needs a Declaration of Performance Shear strength (out of plane) acc.
taking into consideration EN 13986 and the CE-marking. to EN 13353 1,2 to 1,6 N/mm²
For use, the respective national provisions apply.
Shear strength (in plane) acc. to
2 to 5 N/mm²
2.2 Application EN 13353
The main application of the Nordpan-SWP is the decorative Compressive strength parallel 10 to 18 N/mm2
interior construction of buildings. In addition, NORDPAN-SWPs acc. to EN 13353
are used as structural components in structural engineering Compressive strength
10-12 N/mm2
constructions. rectangular acc. to EN 13353
NORDPAN-SWP is also used in the field of door and furniture Tensile strength parallel acc. to
construction. EN 13353
6-12 N/mm2
Tensile strength rectangular acc.
2.3 Technical Data 3 N/mm2
to EN 13353
The performance data of the product are in accordance with the
Declaration of Performance with respect to its essential depending on
characteristics according to EN 13353 and EN 13986. Dimensional deviation geometrical mm
NORDPAN-SWP is produced in accordance with EN 13353 the dimensions
characteristic properties depending on the thickness are given Length < 6 m
in the valid DOP: Width < 2.05 m
Height (min. - max.) 0.010 to 0.060 m
Gross density acc. to EN 13353 430 kg/m3
Surface quality (Possible
characteristic features must be 0, A, B, C -
indicated)
Risk class acc. to DIN 68800-3 4 -
Formaldehyde emissions acc. to
< E1 μg/m3
EN 13986
Thermal conductivity acc. to EN
0.09 - 0.11 W/(mK)
12664
Specific heat capacity acc. to EN
1.6 kJ/kgK
12664
Water vapor diffusion equivalent
air layer thickness acc. to ISO n.r. m
12572
Water vapour diffusion resistance
20 - 50 -
factor acc. to ISO 12572
NORDPAN-SWP is manufactured in accordance with EN13353
from coniferous species, with priority being given to Spruce,
Pine, Larch or Douglas fir. Other coniferous species are
permissible but not typical.
NORDPAN-SWP is produced from kiln-dried coniferous wood
with an average wood moisture content of around 7 % to 9 % at
delivery. For bonding, only approved modern low-emission
adhesives according to chapter 2.5 are used. The mechanical
characteristics of NORDPAN-SWP are in accordance with the
requirements specified in EN 13353. For determining the
2 Environmental Product Declaration - Nordpan GmbH - Srl - Nordpan – Solid wood panels (Update)
technical specifications, the declarations of performance (DOP) resulting exhaust air is cleaned according to the legal
in the currently valid versions apply. The dimensional regulations.
tolerances are defined in accordance with EN 13353. Noise emissions from industrial plants are reduced by structural
The products are manufactured in qualities 0 and A to C in measures and comply with the legal requirements.
accordance with EN 13017-1. The manufacturing process applies to all production facilities
Use of preventive chemical wood preservatives in accordance covered by this EPD.
with DIN 68800-3 is unusual and permitted only if other The employee protection in the manufacturing process
preservative measures given in DIN 68800-2 are not sufficient complies with the respective country-specific requirements,
on their own. employees are provided with personal protective equipment.
2.4 Delivery status 2.8 Product processing/Installation
NORDPAN-SWP is produced with the dimensions according to NORDPAN-SWP can be processed with commercially available
chapter 2.3 and is delivered in accordance with EN13017-1 in tools. The instructions for occupational safety/assembly are to
0-, A-, B- and C-quality. The tolerances according to EN 13353 be observed.
are met.
2.5 Base materials/Ancillary materials 2.9 Packaging
NORDPAN-SWP comprises one to five kiln-dried coniferous To protect NORDPAN-SWP against climatic influences,
bonded single layers. polyethylene foils and wood are used in small quantities during
transportation. In addition, PVC binding material, plastic edge
The following types of adhesive systems are used for bonding protectors (polypropylene), underlay plates (PVC cellular
the individual components (finger jointing and surface bonding): boards) and underlay wood are used as packaging material.
• Melamine-urea-formaldehyde adhesives (MUF)
2.10 Condition of use
• PVAC
The composition of NORDPAN-SWP corresponds to the
NORDPAN-SWP contains of the following proportions of
composition according to Section 2.5 for the entire period of
ingredients per m³ on average:
use.
• Coniferous wood (atro), mainly spruce approx. 88-90 %
• Water approx. 7 - 9 % 2.11 Environment and health during use
• Adhesive about 3 - 5 %, The proportions of the Environmental protection: According to current knowledge, the
adhesives systems used are based on about 90 % MUF intended use of NORDPAN-SWP does not present any hazards
and about 10 % PVAC. or impairments to water, air and soil.
Health protection: Under normal conditions of use, NORDPAN-
The product has an average density of 493 kg/m³. SWP is not expected to cause any damage or impairments to
health.
This product/article/at least one partial article contains NORDPAN-SWP subsequently releases formaldehyde during
substances listed in the candidate list (date: 17.01.2023) life cycle.
exceeding 0.1 percentage by mass: no. NORDPAN-SWP bonded with PVAC based adhesives has
formaldehyde emission values in the range of < 0,01 ppm
This product/article/at least one partial article contains other (ml/m³).
carcinogenic, mutagenic, reprotoxic (CMR) substances in Nordpan-SWP bonded with MUF-based adhesives have low
categories 1A or 1B which are not on the candidate list, emissions of formaldehyde, due to the low level of adhesive in
exceeding 0.1 percentage by mass: no. its internal structure and due to its particular use. Measured
against the limit value of 0.1 ml/m³ (0.124 mg/m³) of the Reach
Biocide products were added to this construction product or it Regulation 1907/2006/EG, the measured values in accordance
has been treated with biocide products (this then concerns a with EN 717-1 can be classified as low.
treated product as defined by the (EU) Ordinance on Biocide NORDPAN-SWP with melamine-based adhesive systems
Products No. 528/2012): no. (MUF) has an emission of formaldehyde in the range of 0.01 to
0.05 ppm (ml/m³).
2.6 Manufacture
NORDPAN-SWP is manufactured from sustainable sawn timber 2.12 Reference service life
(PEFC) sourcing from sustainable forestry. Wet sawn timber is NORDPAN-SWP have been used in structural timber
kiln-dried to a moisture content of about 7 % to 9 %. construction for more than 30 years and is very similar to
To ensure the characteristic values of the NORDPAN-SWP, all Rubner glulam with more than 100 years of experience of use.
individual boards are visually- or machine-graded regarding When used as designated, no end of durability must be
strength and stiffness. expected due to its natural durability (protection against
The graded boards are subsequently assembled to single moisture). When used as designated, the lifetime of
layers (butt or finger jointed) for further production. After NORDPAN-SWP is equal to the duration of use of the building.
applying the adhesive, the single layers are pressed to one to
five-layer blanks. 2.13 Extraordinary effects
After curing of the blanks, the final surface treatment is carried Fire
out by grinding, followed by the format cut of the blanks to NORDPAN-SWP is classified in accordance with 2007/348/EG
obtain the final plate dimension. and EN 13986 as follows:
To ensure the product quality, a treatment with weathering or Fire protection
wood preservatives may be required for transport to the
Name Value
construction site, storage, and during assembly.
Building material class D
2.7 Environment and health during manufacturing Burning droplets d0
During production, there are no negative impacts on water and Smoke gas development s2
soil. The resulting process wastewater is fed into the local
Floor coverings are classified with DFL-s1.
sewage system and cleaned according to legal regulations. The
3 Environmental Product Declaration - Nordpan GmbH - Srl - Nordpan – Solid wood panels (Update)
production of heat and electricity due to the high calorific value
Water of approx. 16.5 MJ/kg (at a humidity of u = 12 %) in compliance
No ingredients are washed out which could be hazardous to with the applicable country-specific requirements
water.
2.15 Disposal
Mechanical destruction If the residues are not used for any other cascading use, waste
The fracture behavior of NORDPAN-SWP is appearance typical wood is disposed according to the applicable country-specific
for solid wood. requirements. Disposal represents a possible but unusual case.
NORDPAN-SWP is assigned to waste code 17 02 01 in the
2.14 Re-use phase European list of waste 2014/955/EU. (Treated NORDPAN-SWP
In the event of selective de-construction, NORDPAN-SWP can is assigned to waste code 17 02 04).
easily be re-used after the end of the structure's service life.
The preferred use of NORDPAN-SWP is in the form of reuse 2.16 Further information
based on the applicable country-specific requirements. More detailed information is available at:
If it is not re-used, it will be subject to thermal utilization for the www.nordpan.rubner.com
3. LCA: Calculation rules
3.1 Declared Unit Module C1 | Deconstruction and demolition
This EPD refers to a declared unit of 1 m³ of solid wood panels After the removal of building components overlying the product,
produced by NORDPAN. The declared unit refers to an average the joints can simply be loosened by screwing or sawing and
density of 493 kg/m³ and a wood moisture at delivery of 9 %. lifted by cranes to the place of removal. Required energy
Declared unit demand can be neglected. The actual energy demand depends
on the installation of the products and can therefore vary
Name Value Unit
greatly in the building context.
Declared unit 1 m3
Gross density 493 kg/m3 Module C2 | Transport to disposal
Wood moisture at delivery 9 % Module C2 includes the transport to waste treatment. In this
case, transport by truck over a transport distance of 50 km is
The analysed products represent an average of one- to five-
assumed.
layered NORDPAN solid wood panels produced at the sites
Strassen (AT) and Olang (IT). The declared unit refers to a
Module C3 | Waste processing
weighted average of both production sites and covers 100 % of
In Module C3, the chipping after the removal of the products is
the production of NORDPAN. It is thus considered a realistic
considered. The wooden products and with them the material-
representation.
inherent properties leave the product system as secondary
combustibles in module C3.
The declared unit was calculated on a volume-weighted basis.
This EPD refers to an average product manufactured at several
Module C4 | Disposal
sites. All products undergo the same processing steps. A
The applied scenario declares the energetic recovery of the
possible variability is expected due to the use of different wood
wooden products, therefore no environmental impacts are to be
species. The upstream chain for spruce is considered
expected from waste processing of the products in C4.
representative.
Module D | Benefits and loads beyond the system
The composition of the boards mainly varies related to the
boundary
binder content. Since the three-layer products represent the
Applying an European average scenario, module D describes
main production share, the representativity of the results is
the energetic recovery of the product at the end of life including
assured. For the single-layer and two-layer panels, an
the corresponding energy substitution potentials.
overestimation of the environmental impact is to be expected.
3.2 System boundary
3.3 Estimates and assumptions
The life cycle assessment of average solid wood panels
All assumptions are verified through detailed documentation
produced by NORDPAN refers to a cradle-to-gate analysis of
and correspond to the best possible representation of reality
the environmental impacts with modules C1–C4 and module D
based on the available data.
(A1–A3 + C + D). The following life cycle phases are part of the
Background data for wood logs refer to generic data for spruce
analysis:
logs in bark derived from GaBi database. Spruce represents the
majority of wood processed at NORDPAN. The used dataset
Module A1–A3 | Production stage
represents an approximation for all other species.
The production stage includes upstream burdens of raw
Regional applicability of the used background data refers to
materials (round wood, lumber, adhesive system, etc.) and the
average data under European or German conditions taken from
corresponding transports to the NORDPAN production sites in
the GaBi database. German data was used for the Austrian and
Olang (IT) and Strassen (AT). Lumber production includes
Italian market whenever European or regionalised average data
direct emissions from drying processes based on a worst-case
were not available.
approximation. Upstream emissions from the use of binding
agents rely on supplier-specific data complemented by
Emissions from wood drying were included in the calculations
secondary data. NORDPAN produces thermal energy in its own
according to Rüter & Diederichs 2012.
biomass boilers at both sites. Strassen is supplied with 100 %
green electricity, Olang is supplied with electricity from the 3.4 Cut-off criteria
Italian grid. Additionally all sites are provided by their own The LCA model covers all available input and output flows,
photovoltaic systems. which can be represented based on robust data and from which
4 Environmental Product Declaration - Nordpan GmbH - Srl - Nordpan – Solid wood panels (Update)
a significant contribution can be expected. Data gaps are filled supplier-specific primary data leading to a high data quality.
with conservative assumptions of average data or generic data
if available and are documented accordingly. Only data with a The technological, geographical and time-related
contribution of less than 1 % were cut off. representativeness of the database was kept in mind when
Thus, no data were neglected, of which a substantial impact is selecting background data. Whenever specific data were
to be expected. All relevant data were collected missing, either generic datasets or representative average data
comprehensively. Cutoff material and energy flows were were used instead. The implemented GaBi background
chosen carefully based on their expected quantitative datasets refer to the latest versions available and are carefully
contribution as well as potential environmental impacts. Thus, it chosen.
can be assumed that the sum of all neglected input flows does
not account for more than 5 % of the total material, water and The assessment of the robustness of the average can be found
energy flows. Environmental impacts of machines, plant and in Section 3.1.
infrastructure were not included.
3.7 Period under review
3.5 Background data Foreground data were collected in the 2022 production year,
This study uses generic background data for the evaluation of and the data are based on the volumes produced on an annual
upstream environmental impacts from GaBi database 2022.2 basis.
as well as recognised literature such as Rüter & Diederichs
2012. 3.8 Geographic Representativeness
Land or region, in which the declared product system is
The analysis of the major amount of adhesives used for the manufactured, used or handled at the end of the product´s
production of solid wood panels is based on primary data from lifespan: Europe
NORDPAN's suppliers. Where necessary, this information was
complemented with estimates ensuring the completeness of the
3.9 Allocation
component's representation in the LCA.
Carbon content and primary energy content of the products
were assessed based on their material inherent properties
3.6 Data quality according to underlying physical relationships.
Data collection is based on product-specific questionnaires. It
3.10 Comparability
follows an iterative process of clarifying questions via e-mail,
Basically, a comparison or an evaluation of EPD data is only
telephone calls or in personal/web meetings. Intensive
possible if all the data sets to be compared were created
discussions between the RUBNER group and Daxner & Merl
according to EN 15804 and the building context, respectively
result in an accurate mapping of product-related material and
the product-specific characteristics of performance, are taken
energy flows. This leads to a high quality of foreground data
into account.
collected. Data collection relies on a consistent process
according to ISO 14044.
The GaBi background database was used to calculate the LCA
(GaBi 10; 2022.2)
The representation of the main binding agents used for the
production of NORDPAN solid wood panels is based on
4. LCA: Scenarios and additional technical information
Characteristic product properties of biogenic carbon
End of life (C1-C4)
During tree growth, the wood assimilates carbon dioxide and
stores biogenic carbon. The carbon stored in the product is Name Value Unit
declared in the following table. Energy recovery 493 kg
Information on describing the biogenic Carbon Content at
Reuse, recovery and/or recycling potentials (D), relevant
factory gate
scenario information
Name ValueUnit
Name Value Unit
kg
Biogenic carbon content in product 219 Processing rate 100 %
C
Efficiency of power plant 68 %
Biogenic carbon content in accompanying kg
2.25
packaging C The product reaches the end-of-waste status after removal from
the building, transport to processing and chipping of the
product. For the end of life of the solid wood panels, energy
recovery as secondary fuel in a biomass power plant is
assumed. As the main sales market for the solid wood products
Installation into the building (A5) is concentrated in the European region, plant-specific
The end of life of the product packaging is not declared in characteristic values correspond to a European average
module A5. scenario (EU). The scenario considers a reprocessing rate of
100 % for the solid wood products after removal from the
Name Value Unit
building. This assumption has to be adjusted accordingly when
Packaging (polyethylene) 0.460 kg
applying the results in the building context. At the end of life of
Packaging (polypropylene) 0.006 kg the product, the equilibrium moisture is comparable to the
Packaging (polyvinyl chloride) 0.299 kg moisture content at delivery. This value can vary depending on
Packaging (wood) 5.031 kg the storage of the product before energy recovery.
The end-of-life scenario used in this LCA study is based on the
following assumptions:
5 Environmental Product Declaration - Nordpan GmbH - Srl - Nordpan – Solid wood panels (Update)
5. LCA: Results
The following table contains the LCA results for a declared unit of 1 m³ of solid wood panels produced by NORDPAN (493 kg/m³).
DESCRIPTION OF THE SYSTEM BOUNDARY (X = INCLUDED IN LCA; MND = MODULE OR INDICATOR NOT DECLARED; MNR
= MODULE NOT RELEVANT)
Benefits and
Construction loads beyond
Product stage Use stage End of life stage
process stage the system
boundaries
la ire ta m w a Ry lp p u s tro p s n a rT g n iru tc a fu n a M e h t m o rf tro p s n a rTe tis e h t o t e ta g y lb m e s s A e s U e c n a n e tn ia M ria p e R tn e m e c a lp e R tn e m h s ib ru fe R y g re n e la n o ita re p Oe s u re ta w la n o ita re p Oe s u n o itc u rts n o c -e Dn o itilo m e d tro p s n a rT g n is s e c o rp e ts a W la s o p s iD -e s u e R-y re v o c e R-g n ilc y c e Rla itn e to p
A1 A2 A3 A4 A5 B1 B2 B3 B4 B5 B6 B7 C1 C2 C3 C4 D
X X X MND MND MND MND MNR MNR MNR MND MND X X X X X
RESULTS OF THE LCA - ENVIRONMENTAL IMPACT according to EN 15804+A2: 1 m³ solid wood panel (493 kg/m³)
Parameter Unit A1-A3 C1 C2 C3 C4 D
Global Warming Potential total (GWP-total) kg CO 2 eq -6.65E+02 0 1.56E+00 8.13E+02 0 -4.36E+02
Global Warming Potential fossil fuels (GWP-fossil) kg CO 2 eq 1.4E+02 0 1.48E+00 3.64E+00 0 -4.09E+02
Global Warming Potential biogenic (GWP-biogenic) kg CO 2 eq -8.06E+02 0 6.47E-02 8.09E+02 0 -2.66E+01
Global Warming Potential luluc (GWP-luluc) kg CO 2 eq 2.51E-01 0 9.97E-03 7.69E-04 0 -4.89E-02
Depletion potential of the stratospheric ozone layer (ODP) kg CFC11 eq 2.69E-09 0 1.45E-13 5.32E-11 0 -3.17E-09
Acidification potential of land and water (AP) mol H+ eq 4.98E-01 0 4.95E-03 7.98E-03 0 3.39E-01
Eutrophication potential aquatic freshwater (EP-freshwater) kg P eq 4.08E-04 0 5.29E-06 1.06E-05 0 -6.39E-04
Eutrophication potential aquatic marine (EP-marine) kg N eq 2.45E-01 0 2.26E-03 1.79E-03 0 7.35E-02
Eutrophication potential terrestrial (EP-terrestrial) mol N eq 2.47E+00 0 2.53E-02 1.88E-02 0 8.71E-01
Formation potential of tropospheric ozone photochemical oxidants kg NMVOC
8.89E-01 0 4.44E-03 4.84E-03 0 3.12E-01
(POCP) eq
Abiotic depletion potential for non fossil resources (ADPE) kg Sb eq 2.99E-05 0 1.49E-07 9.91E-07 0 -6.8E-05
Abiotic depletion potential for fossil resources (ADPF) MJ 2.2E+03 0 1.94E+01 6.6E+01 0 -7.08E+03
m3 world eq
Water use (WDP) 1.33E+01 0 1.66E-02 8.29E-01 0 -2.33E+01
deprived
RESULTS OF THE LCA - INDICATORS TO DESCRIBE RESOURCE USE according to EN 15804+A2: 1 m³ solid wood panel (493
kg/m³)
Parameter Unit A1-A3 C1 C2 C3 C4 D
Renewable primary energy as energy carrier (PERE) MJ 1.07E+03 0 1.35E+00 8.12E+03 0 -2.18E+03
Renewable primary energy resources as material utilization
MJ 8.08E+03 0 0 -8.08E+03 0 0
(PERM)
Total use of renewable primary energy resources (PERT) MJ 9.15E+03 0 1.35E+00 3.66E+01 0 -2.18E+03
Non renewable primary energy as energy carrier (PENRE) MJ 1.86E+03 0 1.95E+01 3.81E+02 0 -7.08E+03
Non renewable primary energy as material utilization (PENRM) MJ 3.4E+02 0 0 -3.15E+02 0 0
Total use of non renewable primary energy resources (PENRT) MJ 2.2E+03 0 1.95E+01 6.6E+01 0 -7.08E+03
Use of secondary material (SM) kg 0 0 0 0 0 0
Use of renewable secondary fuels (RSF) MJ 0 0 0 0 0 8.08E+03
Use of non renewable secondary fuels (NRSF) MJ 0 0 0 0 0 3.15E+02
Use of net fresh water (FW) m3 7.29E-01 0 1.56E-03 3.49E-02 0 -1.49E+00
RESULTS OF THE LCA – WASTE CATEGORIES AND OUTPUT FLOWS according to EN 15804+A2:
1 m³ solid wood panel (493 kg/m³)
Parameter Unit A1-A3 C1 C2 C3 C4 D
Hazardous waste disposed (HWD) kg 6.69E-07 0 1.03E-10 5.71E-09 0 -8.77E-07
Non hazardous waste disposed (NHWD) kg 1.35E+00 0 3.18E-03 4.97E-02 0 2.45E-01
Radioactive waste disposed (RWD) kg 6.38E-02 0 3.62E-05 1.05E-02 0 -6.27E-01
Components for re-use (CRU) kg 0 0 0 0 0 0
Materials for recycling (MFR) kg 0 0 0 0 0 0
Materials for energy recovery (MER) kg 0 0 0 4.93E+02 0 0
Exported electrical energy (EEE) MJ 0 0 0 0 0 0
Exported thermal energy (EET) MJ 0 0 0 0 0 0
RESULTS OF THE LCA – additional impact categories according to EN 15804+A2-optional:
1 m³ solid wood panel (493 kg/m³)
Parameter Unit A1-A3 C1 C2 C3 C4 D
Disease
Incidence of disease due to PM emissions (PM) ND ND ND ND ND ND
incidence
6 Environmental Product Declaration - Nordpan GmbH - Srl - Nordpan – Solid wood panels (Update)
Human exposure efficiency relative to U235 (IR) kBq U235 eq ND ND ND ND ND ND
Comparative toxic unit for ecosystems (ETP-fw) CTUe ND ND ND ND ND ND
Comparative toxic unit for humans (carcinogenic) (HTP-c) CTUh ND ND ND ND ND ND
Comparative toxic unit for humans (noncarcinogenic) (HTP-nc) CTUh ND ND ND ND ND ND
Soil quality index (SQP) SQP ND ND ND ND ND ND
The additional and optional impact categories according to EN 15804+A2 are not declared, as the uncertainty of these indicators is to
be classified as high.
Disclaimer 1 – for the indicator 'Potential Human exposure efficiency relative to U235'.
This impact category deals mainly with the eventual impact of lowdose ionizing radiation on human health of the nuclear fuel cycle. It
does not consider effects due to possible nuclear accidents, occupational exposure or radioactive waste disposal in underground
facilities. Potential ionizing radiation from the soil, from radon and from some construction materials is also not measured by this
indicator.
Disclaimer 2 – for the indicators 'abiotic depletion potential for non-fossil resources', 'abiotic depletion potential for fossil resources',
'water (user) deprivation potential, deprivation-weighted water consumption', 'potential comparative toxic unit for ecosystems', 'potential
comparative toxic unit for humans – cancerogenic', 'Potential comparative toxic unit for humans - not cancerogenic', 'potential soil
quality index'.
The results of this environmental impact indicator shall be used with care as the uncertainties on these results are high as there is
limited experience with the indicator.
6. LCA: Interpretation
The following interpretation contains a summary of the LCA After its use in the building, the product is assumed to be
results referenced to a declared unit of 1 m³ of NORDPAN solid incinerated in a biomass power plant. As a result, the
wood panel. incorporated carbon is emitted again to the atmosphere
representing biogenic carbon dioxide emissions (module C3).
The global warming potential (GWP) of solid wood panels
shows negative values in the production phase (modules A1– The negative values in the end-of-life (module D) result from
A3). These negative impacts result from the use of wood as raw the energetic treatment of the product. As the energy produced
material. Wood sequesters biogenic carbon during tree growth. at the biomass power plant can substitute (mainly fossil) fuels,
The sequestered carbon does not contribute to global warming an environmental net benefit is generated.
as long as it is stored in the biomass.
Potential global warming (GWP) due to the production of wooden residues for heat production. Its thermal treatment is
NORDPAN solid wood panels mainly stems from electricity use taken into account as carbon neutral, as the wood is derived
for production at the Olang site (Italian residual-mix), lumber from sustainably managed forests.
production and the upstream supply chain of the binding
agents. The processing of the products includes the use of all The presented results are considered to be representative for
7 Environmental Product Declaration - Nordpan GmbH - Srl - Nordpan – Solid wood panels (Update)
both NORDPAN production sites. It refers to an average
product based on the weighted production volumes of each Since the wood species processed is dominated by spruce, the
site. variation associated with the forestry of different wood species
is considered to be small.
Due to the different binder contents of specific multi-layer
products, there is a certain variance in the results to be The results of the previous EPD (EPD-RUB-20180061-IBB2-
expected. Three-layer boards account for the majority of the EN) are not directly comparable with the present updated
total production. For single-layer and two-layer boards, tending version due to the update of the underlying methodology
to contain a lower proportion of adhesive, a potential according to EN 15804+A2.
overestimation of the environmental impacts can be assumed.
7. Requisite evidence
The following evidence of environmental and health relevance 53436, no relevant measurement results are available, the test
was provided. specimen geometry is not able to represent the real gas
composition for a representative cross-section.
7.1 Formaldehyde
The emissions (melamine-based adhesive systems) listed in 7.4 VOC emissions
section 2.11 are based on test results of emission For the verification of VOC emissions, two test reports (3-layer:
measurements in accordance with EN 717-1 at a temperature 2519107/4, 2019; 5-layer: 252391/2, 2013) of emission analysis
of 23 °C, a relative humidity of 45 % and an air change rate of according to AgBB-Scheme 2015 are available. Analysis was
1.0 per hour. The test results all meet the requirements of performed in accordance with ISO 16000-9.
emission class E1 according to EN 13986 of 0.124 mg/m³
VOC emissions: 3 layered element: larch
Test report No CT-08-12-17-01, (2008) defines a formaldehyde
Name Value Unit
emission of <0.01 ppm for one layered NORDPAN-SWP with
PVAC adhesive. Overview of Results (28 days) - μg/m3
Test report No 2518056, (2018) defines a formaldehyde TVOC (C6 - C16) acc. to AgBB 2015 8 μg/m3
emission of 0.01 ppm for three layered NORDPAN-SWP with
Sum SVOC (C16 - C22) acc. to AgBB 2015 27 μg/m3
MUF adhesive after 240 h.
R (dimensionless) acc. to AgBB 2015 0,148 -
Test report No PB_2117078_QDF_2021_2, (2021) defines a
formaldehyde emission of 0.02 ppm for three layered The tested specimens fulfil the requirements according to AgBB
NORDPAN-SWP with MUF adhesive after 384 h. Scheme 2015 and French "Arrêté étiquetage".
Test report No CT-14-04-04-02, (2014) defines a formaldehyde
emission of 0.05 ppm for five layered NORDPAN-SWP with
VOC emissions: 5 layered element: spruce
MUF adhesive.
Name Value Unit
According to the test report for proof of occupational exposure
(according to EN 689) (date 23.02.2022), the maximum allowed TVOC (C6 - C16) - μg/m3
workplace concentration of 0.246 mg/m³ is significantly higher Overview of Results (28 days) μg/m³
than the measured concentration of 0.071 mg/m³.
Sum SVOC (C16 - C22) - μg/m3
TVOC (C6 - C16) acc. to /AgBB 2015/ 22 μg/m³
7.2 MDI
In the context of production, no such substances are added to R (dimensionless) - -
the wood. Thus, a MDI emission from the finished NORDPAN- VOC without NIK - μg/m3
SWP is not to be expected.
Carcinogenic Substances - μg/m3
7.3 Fire gas toxicity The tested specimens fulfil the requirements according to AgBB
Due to the heterogeneous structure of NORDPAN-SWP, Scheme 2015 and French "Arrêté étiquetage".
combined with the non-applicability of the test standard DIN
8. References
Standards EN 717-1
DIN EN 717-1:2005-01, Wood-based panels – Determination of
DIN 53436 Formaldehyde release – Part 1: Formaldehyde emission by the
DIN 53436:2015, Generation of thermal decomposition chamber method.
products from materials for their analytic-toxicological testing.
EN 1912
DIN 68800-2 EN 1912:2013-10-15, Structural timber - Strength classes -
DIN 68800-2:2012-02, Wood preservation – Part 2: Preventive Assignment of visual grades and species.
constructional measures in buildings.
EN 12369-3
DIN 68800-3 DIN EN 12369-3:2009-02, Wood-based panels - Characteristic
DIN 68800-3:2012-02, Wood preservation – Part 3: Preventive values for structural design - Part 3: Solid-wood panels.
protection of wood with wood preservatives.
EN 12664
EN 689 EN 12664:2001, Thermal performance of building materials and
EN 689:1995, Workplace atmospheres - Guidance for the products - Determination of thermal resistance by means of
assessment of exposure by guarded hot plate and heat flow meter methods - Dry and moist
inhalation to chemical agents for comparison with limit values products with medium and low thermal resistance.
and measurement strategy.
8 Environmental Product Declaration - Nordpan GmbH - Srl - Nordpan – Solid wood panels (Update)
EN 13183-1 GaBi
EN 13183-1:2002, Moisture content of a piece of sawn timber - GaBi 10, Software-System and Database for Life Cycle
Part 1: Determination by oven dry method. Engineering. 2022.2. Stuttgart, Echterdingen: Sphera, 1992-
2022. Available at: https://sphera.com/product-sustainability-
EN 13353 gabi-data-search/
DIN EN 13353:2011-07, Solid wood panels (SWP) -
Requirements. IBU 2021
Institut Bauen und Umwelt e.V.: General Programme
EN 13986 Instructions for the Preparation of EPDs at the Institut Bauen
DIN EN 13986:2015-06, Wood-based panels for use in und Umwelt e.V. (IBU). Version 2.0, Berlin: Institut Bauen und
construction - Characteristics, evaluation of conformity and Umwelt e.V., 2021. www.ibuepd.com
marking.
Ordinance on Biocide Products
EN 13017-1 Regulation (EU) No 528/2012 of the European Parliament and
DIN EN 13017-1:2001-03, Solid wood panels - Classification by of the Council of 22 May 2012
surface appearance - Part 1: Softwood. concerning the making available on the market and use of
biocidal products.
EN 15804
DIN EN 15804:2012+A2:2019+AC:2021, Sustainability of PCR part A
construction works Environmental product declarations Core Product category rules for building-related products and
rules for the product category of construction products. services. Part A: Calculation Rules for the Life Cycle
Assessment and Requirements on the Project Report according
hEN 14081 to EN 15804+A2:2019. Version 1.3. Berlin: Institut Bauen und
hEN 14081-1:2016-06-01, Timber structures - Strength graded Umwelt e.V., 2022.
structural timber with rectangular cross section - Part 1:
General requirements. PCR: Solid wood products
Product category rules for building-related products and
ISO 12572 services. Part B: EPD requirements for solid wood products.
EN ISO 12572:2016, Hygrothermal performance of building Version v2, Berlin: Institut Bauen und Umwelt e.V., 31.05.2023.
materials and products - Determination of water vapour
transmission properties - Cup method. PCR 305/2011 (EU)
REGULATION (EU) No 305/2011 OF THE EUROPEAN
ISO 14025 PARLIAMENT AND OF THE COUNCIL of 9 March 2011 laying
DIN EN ISO 14025:2011-10, Environmental labels and down harmonised conditions for the marketing of construction
declarations Type III environmental declarations Principles and products and repealing Council Directive 89/106/EEC.
procedures.
Rüter & Diederichs 2012
ISO 14044 Ökobilanz-Basisdaten für Bauprodukte aus Holz. Work report
DIN EN ISO 14044:2006-10, Environmental management - Life from the Institut für Holztechnologie und Holzbiologie Nr.
cycle assessment - Requirements and guidelines. 2012/1. Hamburg: Johann Heinrich von Thünen-Institut.
ISO 16000-9 1907/2006/EG
EN ISO 16000-9:2006, Indoor air - Part 9: Determination of the VERORDNUNG (EG) Nr. 1907/2006 DES EUROPÄISCHEN
emission of volatile organic compounds from building products PARLAMENTS UND DES RATES vom 18. Dezember 2006 zur
and furnishing - Emission test chamber method. Registrierung, Bewertung, Zulassung und Beschränkung
chemischer Stoffe (REACH).
Further references 2007/348/EG
2007/348/EC: Commission Decision of 15 May 2007 amending
AgBB-Scheme 2015 Decision 2003/43/EC establishing the classes of reaction-to-fire
German Committee for HealthRelated Evaluation of Building performance for certain construction products as regards wood-
Products (AgBB): Approach to health assessment of emissions based panels.
of volatile organic compounds (VOCs and SVOCs) from
building products. 2014/955/EU
2014/955/EU, COMMISSION DECISION of 18 December 2014
Candidate List amending Decision 2000/532/EC on the list of waste pursuant
List of substances of very high concern considered for approval to Directive 2008/98/EC of the European Parliament and of the
(status 17.01.2023) according to Article 59 para. 10 of the Council.
REACH Regulation. European Chemicals Agency.
9 Environmental Product Declaration - Nordpan GmbH - Srl - Nordpan – Solid wood panels (Update)
Publisher
Institut Bauen und Umwelt e.V. +49 (0)30 3087748- 0
Hegelplatz 1 info@ibu-epd.com
10117 Berlin www.ibu-epd.com
Germany
Programme holder
Institut Bauen und Umwelt e.V. +49 (0)30 3087748- 0
Hegelplatz 1 info@ibu-epd.com
10117 Berlin www.ibu-epd.com
Germany
Author of the Life Cycle Assessment
Daxner & Merl GmbH +43 676 849477826
Schleifmühlgasse 13/24 office@daxner-merl.com
1040 Wien www.daxner-merl.com
Austria
Owner of the Declaration
Rubner Holding AG - S.p.A. 0039 0474 563 777
Handwerkerzone 2 info@rubner.com
39030 Kiens www.rubner.com
Italy
10 Environmental Product Declaration - Nordpan GmbH - Srl - Nordpan – Solid wood panels (Update)
