ENVIRONMENTAL PRODUCT DECLARATION
as per ISO 14025 and EN 15804+A2
Owner of the Declaration ARGE – The European Federation of Locks and Building Hardware Manufacturers
Publisher Institut Bauen und Umwelt e.V. (IBU)
Programme holder Institut Bauen und Umwelt e.V. (IBU)
Declaration number EPD-ARG-20230543-IBG1-EN
Issue date 02.04.2024
Valid to 01.04.2029
Panic and emergency exit devices
ARGE – The European Federation of Locks
and Building Hardware Manufacturers
This EPD is valid only for products supplied by an ARGE EPD licence holder.
www.ibu-epd.com | https://epd-online.com
1. General Information
ARGE – The European Federation of Locks Panic and emergency exit devices
and Building Hardware Manufacturers
Programme holder Owner of the declaration
IBU – Institut Bauen und Umwelt e.V. ARGE – The European Federation of Locks and Building Hardware
Hegelplatz 1 Manufacturers
10117 Berlin Offerstraße 12
Germany 42551 Velbert
Germany
Declaration number Declared product / declared unit
EPD-ARG-20230543-IBG1-EN 1 kg of panic or emergency exit device
This declaration is based on the product category rules: Scope:
Building Hardware products, 01.08.2021 This ARGE EPD covers panic and emergency exit devices used to enable
(PCR checked and approved by the SVR) rapid and easy egress from buildings. The reference product used to
calculate the impact this product group has on the environment is a panic
exit device composed primarily of steel, Zamak and aluminium, and has
Issue date been selected for the LCA (Life Cycle Assessment) because it is the
product with the highest impact for 1 kg of product. A validity scope
02.04.2024
analysis has also been carried out to determine the limiting factors for
panic and emergency exit devices covered by this EPD. In a preliminary
study (simplified LCA), it has been confirmed that this EPD represents the
Valid to
worst-case condition and it can therefore be used to cover all panic and
01.04.2029 emergency exit devices devices manufactured in Europe by ARGE
member companies.
The owner of the declaration shall be liable for the underlying information
and evidence; the IBU shall not be liable with respect to manufacturer
information, life cycle assessment data and evidences.
The EPD was created according to the specifications of EN 15804+A2. In
the following, the standard will be simplified as EN 15804.
Verification
The standard EN 15804 serves as the core PCR
Independent verification of the declaration and data according to ISO
Dipl.-Ing. Hans Peters
14025:2011
(Chairman of Institut Bauen und Umwelt e.V.)
internally X externally
Florian Pronold Dr. Matthew Fishwick,
(Managing Director Institut Bauen und Umwelt e.V.) (Independent verifier)
1 Environmental Product Declaration - ARGE – The European Federation of Locks and Building Hardware Manufacturers - Panic and emergency exit devices
2. Product
The values are given in the table below are for the product
2.1 Product description/Product definition
analysed for this EPD. Ranges of values for other products
This ARGE EPD covers panic and emergency exit devices covered by the validity scope analysis are shown in brackets
used to allow rapid and easy egress from buildings.
Name Value Unit
For the placing on the market of the product in the European
Steel (36.81% – 77.01%) 36.81 %
Union/European Free Trade Association (EU/EFTA) (with the
exception of Switzerland) Regulation (EU) No. 305/2011 (CPR) Zamak (0.00% – 34.03%) 34.03 %
applies. The product needs a declaration of performance taking Aluminium (22.03% – 25.86%) 25.86 %
into consideration: ABS (0.00% – 1.77%) 1.77 %
• EN 1125:2008, Building hardware – Panic exit devices Nylon 6 (0.00% – 1.53%) 1.53 %
operated by a horizontal bar, for use on escape routes – PVC (0.00% – 0.08%) 0 %
Requirements and test methods.
Brass (0.00% - 0.88%) 0 %
• EN 179:2008, Building hardware – Emergency exit
devices operated by a lever handle or push pad, for use Steel is produced by combining iron with carbon as well as
on escape routes – Requirements and test methods. other elements depending on the desired characteristics.
and the CE-marking. Components made of steel are formed by turning or other types
of mechanical processing.
For the application and use the respective national provisions
apply. Zamak is an alloy with a base metal of zinc and alloying
elements of aluminium, magnesium, and copper. Components
2.2 Application made of Zamak are die-cast.
These products are designed to be integrated into door
assemblies consisting of various materials and used for various Aluminium is a non-ferrous metal produced from bauxite by
applications. They may be used for either interior or exterior the Bayer process. Components made of aluminium are
doors. manufactured by die-casting or other types of mechanical
processing.
2.3 Technical Data
Ideally, products should comply with a suitable technical ABS (acrylonitrile butadiene styrene) is a terpolymer polymer
specification. EN 1125 and EN 179 are examples of such made by polymerizing styrene and acrylonitrile in the presence
specifications and some products will comply with one of these of polybutadiene. Components made of ABS are made by
standards. The relevant grading structure is shown in the injection moulding or other thermal forming processes.
following table:
Name Value Unit Nylon 6 is a polymer, in particular polyamide. It is formed by
Category of use 3 Grade the ring-opening polymerisation of caprolactam. Components
made of Nylon 6 are formed by injection moulding or other
Durability 6, 7 Grade
thermal forming processes.
Door mass 5, 6, 7 Grade
Suitability for use in fire resisting and/or smoke 0, A, B Grade PVC (polyvinyl chloride) is a thermoplastic polymer produced
control doors via polymerisation of vinyl chloride. Components made of PVC
Safety 1 Grade are formed by injection moulding or other thermal forming
Corrosion resistance 3, 4 Grade processes.
Security 2 - 5 Grade
Brass is an alloy of zinc and copper. Components made of
Projection of operating element 1, 2 Grade
brass are made by extrusion, forging, die-casting or other types
Type of operation A, B Grade
of mechanical processing.
A, B, C,
Field of door application Grade
D 1) This product/article/at least one partial article contains
substances listed in the ECHA candidate list (date: 14.06.2023)
Performance data of the product in accordance with the
exceeding 0.1 percentage by mass: Certain components may
declaration of performance with respect to its essential
contain small amounts of lead (CAS no. 7439-92-1) as an
characteristics according to:
alloying element.
• EN 1125:2008, Building hardware – Panic exit devices
operated by a horizontal bar, for use on escape routes -
2) This product/article/at least one partial article contains other
Requirements and test methods cancerogenic, mutagenic, reprotoxic (CMR) substances in
• EN 179:2008, Building hardware – Emergency exit categories 1A or 1B which are not on the ECHA candidate list,
devices operated by a lever handle or push pad, for use exceeding 0.1 percentage by mass: no.
on escape routes - Requirements and test methods
3) Biocide products were added to this construction product or it
2.4 Delivery status
has been treated with biocide products (this then concerns a
The products are sold by unit. Deliveries of individual items are
treated product as defined by the (EU) Ordinance on Biocide
possible but are an exception. Standard deliveries comprise a
Products No. 528/2012): no.
larger quantity of of panic or emergency exit devices, as they
are marketed as "B2B" products and not to end-users. 2.6 Manufacture
The production of a panic and an emergency exit device
2.5 Base materials/Ancillary materials
usually follows a 3-step procedure:
Composition of product analysed for this EPD:
2 Environmental Product Declaration - ARGE – The European Federation of Locks and Building Hardware Manufacturers - Panic and emergency exit devices
1. Manufacture of the components: this step may include
2.12 Reference service life
surface treatment in the factory or by external
The reference service life is 30 years under normal working
contractors.
conditions. This corresponds to passing a mechanical
2. Pre-assembly of modules (in the factory).
endurance test of 200.000 cycles as specified in EN 1125 and
3. Final assembly (in the factory).
EN 179. The reference service life is dependent on the actual
2.7 Environment and health during manufacturing frequency of use and environmental conditions. It is required
Regular measurements of air quality and noise levels are that installation, as well as maintenance of the product, must be
done in line with instructions provided by the manufacturer.
carried out by the manufacturers, the ARGE member
companies. The results shall be within the mandatory safety
2.13 Extraordinary effects
levels. In areas where employees are exposed to chemical
Fire
products, the required protective clothing and technical
In general, both types of products are suitable for use in fire
protective devices shall be provided. Regular health checks are
resisting and/or smoke control door sets according to the
mandatory for employees in production facilities.
classes in EN 1125 and EN 179, unless the product is classified
2.8 Product processing/Installation in class/grade 0.
The installation of the product may vary depending on the type
Water
of door and the specific situation, but the products shall not
The declared product is intended to be used in buildings under
require energy consumption for installation.
normal conditions (indoor or outdoor) They shall not emit
2.9 Packaging hazardous substances in the event of flooding.
Normally, each individual product is packed in paper or
cardboard. These individual products are then packed in a Mechanical destruction
cardboard box and stacked on wooden pallets for transport to Mechanical destruction of the declared product shall not
the customer. materially alter its composition or have any adverse effect on
the environment.
Waste from product packaging is collected separately for waste
2.14 Re-use phase
disposal (including recycling).
Removal of the panic or emergency device (for re-use or
2.10 Condition of use recycling) shall have no adverse effect on the environment.
Once installed, the products shall require no servicing during
2.15 Disposal
their expected service lives. There shall be no consumption of
Components of panic and emergency exit devices should be
water or energy linked to their use, and they shall not cause
recycled wherever possible, providing that there is no adverse
any emissions.
effect on the environment. The waste code in accordance with
2.11 Environment and health during use the European Waste Code is 17 04 07.
No environmental damage or health risks are to be expected
2.16 Further information
during normal conditions of use.
Details of all types and variants can be found on the
manufacturers' websites. The respective website addresses are
available at https://arge.org.
3. LCA: Calculation rules
except for transport and electricity consumption for grinding the
3.1 Declared Unit metals. When recycled metals are used as raw material only
The declared unit for all products covered by this ARGE EPD is their transformation process is taken into account and not the
1 kg (of product). Since individual products will rarely weigh extraction of the raw material.
exactly 1 kg it is necessary to establish the exact weight of the A4 module represents the transport of the finished panic exit
product and then use this as a correction factor to determine device to the installation site.
the true values for 1 kg of product in the tables (Section 5). There is no waste associated with the installation of the
Declared unit product. The A5 module therefore represents only the disposal
of the product packaging.
Name Value Unit
The End-of-Life (EoL) stages are also considered. The
Declared unit 1 kg
transportation to the EoL disposal site is taken into account in
Mass of declared product 1.95 kg module C2. Module C4 covers the disposal of the locks. Module
Raw density 1 kg/m3 C3 covers the recycling of the individual elements according to
European averages, with the remaining waste divided between
incineration and landfill. Such a mixed scenario is declared due
to the complex material mix of the product and the dependency
3.2 System boundary
of the EoL-route on the EoL-route of the product the panic exit
Type of the EPD: "cradle to gate with options, with modules C1
device has been integrated into.
– C4, and module D (A1-A3, C1-C3, D and additional
In practice, the end of life has been modelled as follows:
modules)"
• when a material is sent for recycling, generic transport
The analysis of the product life cycle includes the production and electric consumption of a shredder is taken into
and transport of the raw materials, the manufacture of the account (corresponding to the process 'Grinding,
product and the packaging materials which are declared in metals'). Only then, is the material considered to have
modules A1-A3. attained the 'end-of-waste' state.
Losses during production are considered as waste and are sent • each type of waste is modelled as a transport to the
for recycling. No recycling processes are taken into account treatment site with a distance of 30 km. Parts sent for
3 Environmental Product Declaration - ARGE – The European Federation of Locks and Building Hardware Manufacturers - Panic and emergency exit devices
recycling include electricity consumption (grinding) and • In the absence of collected data, generic data from the
a flow ('Materials for recycling, unspecified'). ecoinvent v3.8 database have been used. This is
updated regularly and is representative of current
3.3 Estimates and assumptions processes (the entire database having been updated in
The LCA data of the declared panic exit device have been 2021).
calculated from the production data of one ARGE member Geography: Data come from production sites of the ARGE
company, representing 2 different kinds of product. This member companies. Generic data come from the ecoinvent
company was chosen by ARGE as being representative by database, representative for European production processes.
means of its production process and its market share. The
product chosen as representative for this calculation follows the Technology: Material shaping technologies are based on
"worst-case" principle as explained in section 6. LCA European technology in the case of the use of generic data.
interpretation.
A total of 2 typical products (based on sales figures) have been
3.4 Cut-off criteria
evaluated, and the worst-case results are used in the tables.
The cut-off criteria considered are 1% of renewable and non-
renewable primary energy usage and 1% of the total mass of 3.7 Period under review
that unit process. The total neglected input flows per module The data of the LCA is based on the annual production data of
shall be a maximum of 5% of energy usage and mass. an ARGE member from 2013, considered representative for the
year 2022.
For this study, all input and output flows have been considered
at 100%, including raw materials as per the product 3.8 Geographic Representativeness
composition provided by the manufacturer and packaging of Land or region, in which the declared product system is
raw materials as well as the final product. Energy and water manufactured, used or handled at the end of the product´s
consumptions have also been considered at 100% according to lifespan: Europe
the data provided.
3.9 Allocation
With the approach chosen, no significant environmental
impacts are known to have been cut off. The products covered by this EPD are produced on one
production site. All data were provided by the manufacturer of
3.5 Background data the products per unit and then divided by the mass of the
For the life cycle modelling of the considered product, all product to give a value per kg of product produced.
relevant background datasets are taken from ecoinvent v3.8
(system model: cut-off by classification). The assumptions relating to the EoL of the product are
described in the section System Boundaries.
3.6 Data quality
The objective of this evaluation is to evaluate the environmental Metal losses during production (stage A3) are considered as
impacts generated by the products throughout their entire life waste.
cycles. To this end, ISO 14040, ISO 14044 and EN 15804 have
been met regarding the quality of data on the following different 3.10 Comparability
criteria: Basically, a comparison or an evaluation of EPD data is only
possible if all the data sets to be compared were created
Time: The life cycle inventory data used come from: according to EN 15804 and the building context, respectively
the product-specific characteristics of performance, are taken
• Data collected specifically for this study on the ARGE
into account.
member companies' manufacturing sites. Datasets are
based on 1-year averaged data (time period: January
ecoinvent v3.8 (system model: cut-off by classification) has
2013 to December 2013 considered representative for
been used as the background database.
2022).
4. LCA: Scenarios and additional technical information
Name Value Unit
Characteristic product properties of biogenic carbon
Litres of fuel 25.8 l/100km
Transport distance 3500 km
Information on the biogenic carbon content at factory gate
Capacity utilisation (including empty runs) 36 %
Note: 1 kg of biogenic carbon is equivalent to 44/12 kg of CO 2.
Name Value Unit Installation into the building (A5)
kg Name Value Unit
Biogenic carbon content in product 0
C Material loss 0.144 kg
Biogenic carbon content in accompanying kg
0.0570
packaging C
Reference service life
Name Value Unit
The following information is the basis of the declared modules
Reference service life (condition of use: see
within the LCA in this EPD. 30 a
§2.13)
Transport to the building site (A4)
Test cycles over RSL (EN 1125, EN 179) 200'000 cycles
End of life (C1-C4)
4 Environmental Product Declaration - ARGE – The European Federation of Locks and Building Hardware Manufacturers - Panic and emergency exit devices
Name Value Unit output flow.
Collected separately waste type 1 kg
For building hardware, the following rules apply for the
Recycling 0.475 kg
quantification of net output flows:
Energy recovery 0.242 kg
- all production scrap and cuttings leave modules A1-B3 as
Landfilling 0.284 kg sorted scrap without allocated burdens from primary production;
the corresponding amounts are declared as material for
It is assumed that a 16–32-ton truck is used to transport the
recycling (MFR);
product:
- net amounts of a metal leaving the product system are
- Transport to shredding facility for metal recovery: 150 km
quantified as the material for recycling leaving modules A1-C4
- Transport to municipal waste incineration plant: 50 km
minus the input of secondary scrap (secondary material, SM) to
- Transport to landfill: 30 km
the product system;
- in the case of brass and zinc alloys, which are composed of
two different constituting metals, no difference shall be made
Reuse, recovery and/or recycling potentials (D), relevant
between the input of secondary constituting metals (Cu and Zn;
scenario information
Cu and Sn) and its alloys (CuZn; CuSn).
Module D contains the benefits and loads beyond the system
Negative net output flows have not been considered in the
boundary related to the recycling of metals, which result from
quantification of module D.
the treatment of recycled materials from the point of end-of-
waste status to the point of substitution (as costs) and the
It also includes the benefits and loads related to 'exported
substitution of primary resources (as benefits).
energy electricity' and 'expo rtedenergy heat' resulting from the
energy recovery from plastic wastes in a municipal waste
According to EN 16710, clause 6.4.3.3: 'In module D
incineration plant as modelled in Modules A3, A5 and C4.
substitution effects are calculated only for the resulting net
5 Environmental Product Declaration - ARGE – The European Federation of Locks and Building Hardware Manufacturers - Panic and emergency exit devices
5. LCA: Results
In Table 1 "Description of the system boundary", the declared modules are indicated with an "X"; all modules that are not declared
within the EPD but where additional data are available are indicated with "MND". Those data can also be used for building assessment
scenarios. The values are declared with three valid digits in exponential form.
The set of characterisation factors EF3.0 has been used for the life cycle assessment.
DESCRIPTION OF THE SYSTEM BOUNDARY (X = INCLUDED IN LCA; MND = MODULE OR INDICATOR NOT DECLARED; MNR
= MODULE NOT RELEVANT)
Benefits and
Construction loads beyond
Product stage Use stage End of life stage
process stage the system
boundaries
la ire wta am R y lp p u s tro p s n a rT g n iru tc a fu n a M tro p s nm ae o rh r
T
f t e ot ti s e e tah gt y lb m e s s A e s U e c n a n e tn ia M ria p e R tn e m e c a lp e R tn e m h s ib ru fe R la n o ity ag rr ee pn Oe e s u la n o ita r re et pa Ow e s u n o itc u rts n eo Dc -n o itilo m e d tro p s n a rT g n is s ee tsc ao Wrp la s o p s iD e s u e R- y re v o c e R- g n ilc y c e R- la itn e to p
A1 A2 A3 A4 A5 B1 B2 B3 B4 B5 B6 B7 C1 C2 C3 C4 D
X X X X X MND MND MNR MNR MNR MND MND X X X X X
RESULTS OF THE LCA - ENVIRONMENTAL IMPACT according to EN 15804+A2: 1 kg of emergency exit and panic exit devices
Parameter Unit A1-A3 A4 A5 C1 C2 C3 C4 D
GWP-total kg CO2 eq 3.24E+01 6.52E-01 2.32E-01 0 1.64E-02 3.63E-03 3.66E-02 -2.5E+00
GWP-fossil kg CO2 eq 3.25E+01 6.52E-01 2.33E-02 0 1.64E-02 3.62E-03 3.66E-02 -2.49E+00
GWP-biogenic kg CO2 eq -2.09E-01 0 2.09E-01 0 0 0 0 0
GWP-luluc kg CO2 eq 5.21E-02 2.61E-04 1.24E-06 0 6.55E-06 9.04E-06 3.38E-06 -6.56E-03
ODP kg CFC11 eq 2.04E-06 1.51E-07 6.91E-10 0 3.79E-09 1.84E-10 1.32E-09 -9.19E-08
AP mol H+ eq 1.65E-01 1.85E-03 1.72E-05 0 4.65E-05 1.87E-05 3.75E-05 -1.78E-02
EP-freshwater kg P eq 1.66E-03 4.65E-06 2.96E-08 0 1.17E-07 4.07E-07 7.72E-08 -1.14E-04
EP-marine kg N eq 3.59E-02 3.68E-04 6.11E-06 0 9.24E-06 2.39E-06 1.45E-05 -2.46E-03
EP-terrestrial mol N eq 2.99E-01 4.1E-03 6.6E-05 0 1.03E-04 2.77E-05 1.49E-04 -2.77E-02
kg NMVOC
POCP 1.5E-01 1.58E-03 1.85E-05 0 3.96E-05 7.57E-06 4.35E-05 -9.3E-03
eq
ADPE kg Sb eq 8.01E-04 2.31E-06 1.14E-08 0 5.8E-08 8.78E-09 1.96E-08 -2.94E-04
ADPF MJ 4.22E+02 9.89E+00 4.76E-02 0 2.48E-01 7.68E-02 9.2E-02 -2.36E+01
m3 world eq
WDP 1.12E+01 3.01E-02 3E-04 0 7.56E-04 8.58E-04 -6.46E-04 -4.62E-01
deprived
GWP = Global warming potential; ODP = Depletion potential of the stratospheric ozone layer; AP = Acidification potential of land and water; EP =
Eutrophication potential; POCP = Formation potential of tropospheric ozone photochemical oxidants; ADPE = Abiotic depletion potential for non-fossil
resources; ADPF = Abiotic depletion potential for fossil resources; WDP = Water (user) deprivation potential)
RESULTS OF THE LCA - INDICATORS TO DESCRIBE RESOURCE USE according to EN 15804+A2: 1 kg of emergency exit and
panic exit devices
Parameter Unit A1-A3 A4 A5 C1 C2 C3 C4 D
PERE MJ 3.92E+01 1.39E-01 -7.08E-01 0 3.49E-03 1.46E-02 5.03E-03 -2.81E+00
PERM MJ 1.78E+00 0 -2.15E-01 0 0 0 0 0
PERT MJ 4.1E+01 1.39E-01 -9.23E-01 0 3.49E-03 1.46E-02 5.03E-03 -2.81E+00
PENRE MJ 4.22E+02 9.89E+00 3.38E-01 0 2.48E-01 7.75E-02 5.63E-01 -2.36E+01
PENRM MJ 1.31E+00 0 -2.9E-01 0 0 0 -4.71E-01 0
PENRT MJ 4.23E+02 9.89E+00 4.76E-02 0 2.48E-01 7.75E-02 9.2E-02 -2.36E+01
SM kg 3.27E-01 0 0 0 0 0 0 0
RSF MJ 0 0 0 0 0 0 0 0
NRSF MJ 0 0 0 0 0 0 0 0
FW m3 3.5E-01 1.05E-03 5.19E-05 0 2.63E-05 4.95E-05 1.99E-04 -1.79E-02
PERE = Use of renewable primary energy excluding renewable primary energy resources used as raw materials; PERM = Use of renewable primary
energy resources used as raw materials; PERT = Total use of renewable primary energy resources; PENRE = Use of non-renewable primary energy
excluding non-renewable primary energy resources used as raw materials; PENRM = Use of non-renewable primary energy resources used as raw
materials; PENRT = Total use of non-renewable primary energy resources; SM = Use of secondary material; RSF = Use of renewable secondary fuels;
NRSF = Use of non-renewable secondary fuels; FW = Use of net fresh water
RESULTS OF THE LCA – WASTE CATEGORIES AND OUTPUT FLOWS according to EN 15804+A2:
1 kg of emergency exit and panic exit devices
Parameter Unit A1-A3 A4 A5 C1 C2 C3 C4 D
HWD kg 2.71E-02 2.58E-05 2.15E-07 0 6.48E-07 2.72E-08 1.74E-07 6.97E-05
NHWD kg 6.52E+00 5.2E-01 3.19E-03 0 1.31E-02 2.89E-04 3.33E-01 -6.69E-01
RWD kg 2.1E-03 1.43E-04 6.17E-07 0 3.59E-06 1.03E-06 1.16E-06 -6.53E-05
CRU kg 0 0 0 0 0 0 0 0
MFR kg 3.54E-01 0 9.3E-02 0 0 5.43E-01 0 0
6 Environmental Product Declaration - ARGE – The European Federation of Locks and Building Hardware Manufacturers - Panic and emergency exit devices
MER kg 0 0 0 0 0 0 0 0
EEE MJ 0 0 3.71E-02 0 0 0 2E-02 0
EET MJ 0 0 2.45E-01 0 0 0 1.32E-01 0
HWD = Hazardous waste disposed; NHWD = Non-hazardous waste disposed; RWD = Radioactive waste disposed; CRU = Components for re-use;
MFR = Materials for recycling; MER = Materials for energy recovery; EEE = Exported electrical energy; EET = Exported thermal energy
RESULTS OF THE LCA – additional impact categories according to EN 15804+A2-optional:
1 kg of emergency exit and panic exit devices
Parameter Unit A1-A3 A4 A5 C1 C2 C3 C4 D
Disease
PM 1.46E-06 5.24E-08 3E-10 0 1.32E-09 4.99E-11 9.14E-10 -1.8E-07
incidence
IR kBq U235 eq 1.43E+00 4.29E-02 1.88E-04 0 1.08E-03 7E-04 4.06E-04 -2.77E-02
ETP-fw CTUe 8.64E+02 7.76E+00 4.49E-02 0 1.95E-01 3.86E-02 3.73E+01 -1.12E+02
HTP-c CTUh 3.32E-08 2.5E-10 3.37E-12 0 6.27E-12 1.03E-12 1.5E-11 -2.7E-09
HTP-nc CTUh 8.77E-07 7.84E-09 1.37E-10 0 1.97E-10 3.35E-11 1.64E-10 -9.92E-08
SQP SQP 1.05E+02 6.89E+00 3.03E-02 0 1.73E-01 1.18E-02 1.56E-01 -7.73E+00
PM = Potential incidence of disease due to PM emissions; IR = Potential Human exposure efficiency relative to U235; ETP-fw = Potential comparative
Toxic Unit for ecosystems; HTP-c = Potential comparative Toxic Unit for humans (cancerogenic); HTP-nc = Potential comparative Toxic Unit for humans
(not cancerogenic); SQP = Potential soil quality index
Disclaimer 1 – for the indicator 'Potential Human exposure efficiency relative to U235'. This impact category deals mainly with the
eventual impact of low-dose ionizing radiation on human health of the nuclear fuel cycle. It does not consider effects due to possible
nuclear accidents, occupational exposure or radioactive waste disposal in underground facilities. Potential ionizing radiation from the
soil, radon and from some construction materials is also not measured by this indicator.
Disclaimer 2 – for the indicators 'abiotic depletion potential for non-fossil resources', 'abiotic depletion potential for fossil resources',
'water (user) deprivation potential, deprivation-weighted water consumption', 'potential comparative toxic unit for ecosystems', 'potential
comparative toxic unit for humans – cancerogenic', 'Potential comparative toxic unit for humans - not cancerogenic', 'potential soil
quality index'. The results of this environmental impact indicator shall be used with care as the uncertainties on these results are high
as there is limited experience with the indicator.
6. LCA: Interpretation
Figure 1 illustrates the relative contributions of the different
modules along the life cycle of the declared products.
significant.
Figure 1: Environmental impacts of panic and emergency
exit devices along its life cycle Benefits and burdens beyond the system boundary (module D)
are in the order of 5 % to 25% of the impacts over the product
The largest part of environmental impacts is caused during life cycle (modules A1-A3) and relate basically to the recycling
production (modules A1-A3); comparably small impacts are of metals.
caused during the transport of the product to the construction
site (via the manufacturer of the product, which the panic exit A total of 2 typical products (based on sales figures) have been
device has been integrated into). evaluated and the worst-case results are used in section 5 of
this EPD. In chapter 2.5, the tabulated range of relative weight
All the other modules related to the product life cycle are not per material ensures that the variability of results stays within
7 Environmental Product Declaration - ARGE – The European Federation of Locks and Building Hardware Manufacturers - Panic and emergency exit devices
+/- 40% of the declared values (assessed for the indicators GWP, PENRT, and non-hazardous waste).
7. Requisite evidence
No testing results are required by the PCR part B.
8. References
Product category rules of IBU operated by a lever handle or push pad, for use on escape
routes - Requirements and test methods.
IBU (2021)
IBU (2021): General Instructions for the EPD Programme of the EN 13501-1
Institut Bauen und Umwelt e.V. (General Instructions for the EN 13501-1:2018, Fire classification of construction products
IBU EPD Programme). Version 2.0, Institut Bauen und Umwelt, and building elements - Part 1: Classification using data from
Berlin. reaction to fire tests.
IBU (2021) ISO 15686
IBU (2021): PCR Part A: Calculation rules for the life cycle ISO 15686:1, -2, -7 and -8. Service life planning (various parts).
assessment and requirements on the project report according
to EN 15804+A2. Version 1.3., Institut Bauen und Umwelt, Regulation No. 305/2011
Berlin. Regulation No. 305/2011 (Construction Products Regulation, or
CPR) of the European Parliament and of the European Council
IBU (2023) is a regulation of 9 March 2011 that lays down harmonised
IBU (2023): PCR Part B: Requirements on the EPD for building conditions for the marketing of construction products and
hardware products, Institut Bauen und Umwelt, Berlin. replaces Construction Products Directive (89/106/EEC).
Standards and legal documents ECHA candidate list
Candidate List of substances of very high concern for
EN 15804 Authorisation, published in accordance with Article 59(10) of the
EN 15804:2012+A2:2019+AC:2021, Sustainability of REACH Regulation. European Chemicals Agency, Brussels.
construction works - Environmental product declarations - Core
rules for the product category of construction products. Ordinance on Biocide Products No. 528/2012
REGULATION (EU) No 528/2012 OF THE EUROPEAN
EN 17610 PARLIAMENT AND OF THE COUNCIL of 22 May 2012
EN 17610:2022, Building hardware - Environmental product concerning the making available on the market and use of
declarations - Product category rules complementary to EN biocidal products.
15804 for building hardware.
European List of Waste
ISO 14025 Commission Decision of 3 May 2000 replacing Decision
ISO 14025:2006-07, Environmental labels and declarations - 94/3/EC establishing a list of wastes pursuant to Article 1(a) of
Type III Environmental declarations - Principles and Council Directive 75/442/EEC on waste and Council Decision
procedures. 94/904/EC establishing a list of hazardous waste pursuant to
Article 1(4) of Council Directive 91/689/EEC on hazardous
ISO 14044 waste (notified under document number C(2000) 1147).
EN ISO 14044:2006-07, Environmental management - Life
cycle assessment - Requirements and guidance (ISO Additional references
14044:2006); German and English versions EN ISO
14044:2006. BBSR 2017
BBSR (2017): Nutzungsdauer von Bauteilen in
EN 1125 Lebenszyklusanalysen nach Bewertungssystem Nachhaltiges
EN 1125:2008,Building hardware - Panic exit devices operated Bauen (BNB). Version vom 24.10.2017, Bundesinstitut für Bau-,
by a horizontal bar, for use on escape routes - Requirements Stadt- und Raumforschung, Berlin.
and test methods.
ecoinvent v3.8
EN 179 http://www.ecoinvent.org
EN 179:2008, Building hardware - Emergency exit devices
8 Environmental Product Declaration - ARGE – The European Federation of Locks and Building Hardware Manufacturers - Panic and emergency exit devices
Publisher
Institut Bauen und Umwelt e.V. +49 (0)30 3087748- 0
Hegelplatz 1 info@ibu-epd.com
10117 Berlin www.ibu-epd.com
Germany
Programme holder
Institut Bauen und Umwelt e.V. +49 (0)30 3087748- 0
Hegelplatz 1 info@ibu-epd.com
10117 Berlin www.ibu-epd.com
Germany
Author of the Life Cycle Assessment
Dr. Frank Werner - Umwelt & Entwicklung + 41 (0)44 241 39 06
Kammelenbergstrasse 30 frank@frankwerner.ch
9011 St. Gallen http://www.frankwerner.ch/
Switzerland
Owner of the Declaration
ARGE – The European Federation of Locks and +49 (0)2051 9506 15
Building Hardware Manufacturers mail@arge.org
Offerstraße 12 www.arge.org
42551 Velbert
Germany
9 Environmental Product Declaration - ARGE – The European Federation of Locks and Building Hardware Manufacturers - Panic and emergency exit devices
