Environmental Product Declaration
In accordance with 14025 and EN15804 +A2
PAROC LT Produced Stone Wool Thermal Insulation
Owner of the declaration: Program holder and publisher:
Paroc Group Oy The Norwegian EPD foundation
Product name: Declaration number:
PAROC LT Produced Stone Wool Thermal NEPD-4339-3565-EN
Insulation
Registration number:
Declared unit: NEPD-4339-3565-EN
1 m2 of stone wool with a thermal resistance of
1 m2K/W.
Issue date: 05.04.2023
Product category /PCR: Valid to: 05.04.2028
CEN Standard EN 15804+A2 serves as core
PCR. NPCR PART A Construction Products and
Services NPCR 012 Part B for Thermal
The Norwegian Insulation Products. Updated 04.03.2024
EPD Foundation
General information
Product: Owner of the declaration:
PAROC LT Produced Stone Wool Thermal Insulation Paroc Group Oy
Contact person: Emelia Samuelsson
Phone: +358 46 876 8000
Program Operator:
e-mail: InsulationEurope.Sustainability@owenscorning.com
The Norwegian EPD Foundation
Post Box 5250 Majorstuen, 0303 Oslo, Norway
Tlf: +47 23 08 80 00
e-mail: post@epd-norge.no
Manufacturer:
Paroc Group Oy
Declaration Number:
FI-00181, Helsinki, Finland
Phone: +358 46 876 8000
e-mail: InsulationEurope.Sustainability@owenscorning.com
NEPD-4339-3565-EN
This declaration is based on Product
Category Rules: Place of production:
CEN Standard EN 15804+A2 serves as core PCR. NPCR Vilnius, Lithuania
PART A Construction Products and Services NPCR 012
Part B for Thermal Insulation Products. Management system:
ISO 9001 and ISO 14001
Statements:
The owner of the declaration shall be liable for the Organisation no:
underlying information and evidence. EPD Norway
887294852
shall not be liable with respect to manufacturer, life
cycle assessment data and evidence.
Issue date:
Declared unit:
1 m² of stone wool with a thermal resistance (R of 1 05.04.2023
Valid to:
m2K/W.
Declared unit with option:
05.04.2028
Year of study:
2021
Functional unit:
1 m² of stone wool with thermal resistance (R of 1
m2K/W. 1 m2 of the reference product, PAROC Ultra, at Comparability:
R=1 is at a weight of 1,15 kg. The impact excludes any EPDs from other programmes than EPD Norway
lamination.
may not be comparable.
Verification: The EPD has been worked out by:
Independent verification of the declaration and Emelia Samuelsson, Owens Corning
data, according to ISO14025:2010
internal external x
Approved
Martin Erlandsson, IVL
Independent verifier approved by EPD Norway
Manager of EPD Norway
EPD for the best environmental decision 2
Product
Product description:
PAROC® stone wool insulation in naturally non-combustible and durable. It is made of natural
stone (~98%) and air (~2%). As stone wools thermal performance is based on static air,
insulation products keep their energy saving abilities and dimensions in different temperature
and moisture conditions during the life cycle of a building.
The products covered by this declaration are PAROC stone wool thermal insulation products
manufactured in Vilnius, Lithuania using cupola furnaces.
Product specification:
The average composition used for this EPD is calculated based on line consumption figures for
raw materials. The raw materials are mainly natural stones and resin binder.
Materials %
Stone Wool Fiber >94
Binder (phenol-formaldehyde-urea-copolymer) <6
Dustbinding (mineral oil) <1
Technical data:
For the products covered by this EPD, the performance data are in accordance with the
declaration of performance with respect to its essential characteristics according to EN
13162:2012+A1:2015, "Thermal insulation products for buildings – Factory made mineral wool
(MW) products – Specification."
- Thermal conductivity: 0,033-0,044 W/mK, EN 12939 and EN 12667
- Fire class: A1, EN 13501-1:2007+A1:2009
Complete technical specifications can be found on www.paroc.com
Market:
This EPD is intended for the markets that receives PAROC building insulation products from the
factory in Vilnius, Lithuania. Those markets are mainly Lithuania, Latvia, Estonia, Poland and
Ukraine.
Reference service life, product:
The reference service life of PAROC products is equal to the reference service life of the
building. For the purpose of this EPD the reference service life if considered to be minimum 60
years, which is usually the assumption about the lifetime of the building where this is installed.
Reference service life, building:
The reference service life of a building is set to 60 years in this EPD.
EPD for the best environmental decision 3
LCA: Calculation rules
Declared unit:
The declared unit refers to 1 m2 of PAROC Ultra with a thermal resistance (R) of 1 m2K/W,
thickness of 35 mm and weight of 1,15 kg.
The specific product, PAROC Ultra, is a stone wool slab with a density of 32,8 kg/m3 and
thickness of 100 mm.
The impact indicators for another product can be calculated by multiplying the results of the
EPD with the respective scaling factor for the products covered by this EPD. A table with the
products available in the scaling table and their respective scaling factors is provided within the
‘Additional technical information’ section.
Data quality:
All primary data are collected line specific, based on the financial year 2021. The production
data from Vilnius involves production lines with cupola furnaces.
The background data has been taken from the latest available GaBi database (/GaBi TS) CUP
2022.2. The requiremens for data quality and background data correspond to the specificiations
of EN 15804+A2. The process data and the used background data are consistent.
The data quality can be qualified as good.
Allocation:
The allocation correspond to the specifications of EN 15804+A2. Allocation and other
methodological choices are made consistently throughout the model. As a worst-case approach,
price allocation is considered for the plant.
EPD for the best environmental decision 4
System boundary:
The system boundary of the EPD follows the modular structure defined by EN15804+A2. The
flowchart above represents the system boundaries for the product, construction process, end-
of-life and benefits (D). The use stage (B1-B7) relating to the building site is not included in this
study, as there are no activites and no significant environmental impact in the use stage.
Cut-off criteria:
All data from the production data acquisition has been considered, i. e. all basic materials used
per formulation, utilized thermal energy, internal fuel consumption and electric power
consumption, direct production waste, and all emission measurements available. All material
and energy flows, except paper for labels in packaging, with a proportion of less than 1% have
been considered. The neglected flow (paper label for packaging) does not exceed 1% of the
impact categories. Machines and facilities required during production are neglected.
The declared unit of stone wool is without any coating.
EPD for the best environmental decision 5
LCA: Scenarios and additional technical information
The following information describe the scenarios in the different modules of the EPD. There are
no maintenance (B2), repair (B3), replacements (B4) or refurbishments (B5) required during
the use of PAROC stone wool thermal insulation products in standard conditions. They do not
require energy (B6) or water (B7) during their operational life. No significant emissions to the
indoor environment occur in module (B1). Therefore, modules B1-B7 are not relevant for this
EPD.
Transport from production place to assembly/user (A4)
Fuel/Energy value
Capacity utilisation (incl. Type of
Type Distance KM consumption (l/t for total
return) % vehicle
(l/t.km) distance)
Truck, Euro
Truck 30 5, 27 t 120 0,006 0,72
payload
The A4 distance is calculated as average distance for the Lithuanian market.
Assembly (A5)
Unit Value
Auxiliary kg 0,00
Water consumption m3 0,00
Electricity consumption kWh 0,00
Other energy carriers MJ 0,00
Material loss kg 0,02
Output materials from waste treatment kg 0,08
Dust in the air kg 0,00
The installation in general takes place manually. Thus, machines or energy expenditures are not
taken into account. Most products are self-supporting and do not need support. Installation
losses have been accounted for 2% as a conservative approach. Within module A5 a site related
packaging waste processing is included in the LCA. It is assumed that packaging material as
leftover of the installed product is for 100% collected and incinerated.
End of Life (C1, C3, C4)
Unit Value
kg 0,00
Hazardous waste disposed
kg 0,00
Collected as mixed construction waste
kg 0,00
Reuse
kg 0,00
Recycling
kg 0,00
Energy recovery
kg 1
To landfill
EPD for the best environmental decision 6
Although mineral wool products from Paroc can be recycled, they are estimated as being 100%
landfilled after the use phase as the most conervative approach.
Transport to waste processing (C2)
Fuel/Energy value
Capacity utilisation (incl. Type of
Type Distance KM consumption (l/t for total
return) % vehicle
(l/t.km) distance)
Truck, Euro
Truck 50 5, 27 t 50 0,006 0,30
payload
The distance representes an average distance to landfill, the stone wool is in general not
transported alone to landfill, therefore a load factor of 50% is considered in this case.
Benefits and loads beyond the system boundaries (D)
Benefits are considered in module D for the thermal and electrical energy, generated in module
A5, due to thermal treatment of packaging waste (polyethylene film and wooden pallets) after
installation.
Additional technical information
Below a list of products covered by this EPD and their scaling factors. The scaling factor can be
used to estimate the environmental performance indicators for the specific products of 1 m2
when R=1. The environmental performance solely refer to the stone wool, and thus do not
include the environmental performance of any potential coatings. Due to this fact, the variation
is less than 10% by reason of the density, lambda and binder. The scaling calculation shall be
done as follows:
Reference product environmental impact per m2 (1,31) x scaling factor of specific product
(1,00)
Product Group Product Name Unit Value
PAROC Ultra (42-200 mm thickness, lambda 0,035, average
Flexible Slabs & Mats 1 m2 1,00
density 32,8 kg/m3)
PAROC Ultra plus (50-200 mm thickness, lambda 0,034,
Flexible Slabs & Mats 1 m2 1,24
average density 42 kg/m3)
PAROC Solid (50-180 mm thickness, lambda 0,037, average
Flexible Slabs & Mats 1 m2 0,96
density 29,9 kg/m3)
PAROC Sonus (75-100 mm thickness, lambda 0,044, average
Flexible Slabs & Mats 1 m2 0,92
density 24 kg/m3)
PAROC ROS 30 (50-200 mm thickness, lambda 0,036, average
Roofs 1 m2 3,01
density 96 kg/m3)
PAROC ROS50 (40-150 mm thickness, lambda 0,038, average
Roofs 1 m2 4,09
density 123,5 kg/m3)
PAROC ROS60 (40-50 mm thickness, lambda 0,039, average
Roofs 1 m2 4,42
density 130 kg/m3)
PAROC ROS70 (40-150 mm thickness, lambda 0,039, average
Roofs 1 m2 4,62
density 136 kg/m3)
PAROC ROL 30 (170-360 mm thickness, lambda 0,038,
Roofs 1 m2 2,15
average density 65 kg/m3)
PAROC ROB50 (20-30 mm thickness, lambda 0,037, average
Roofs 1 m2 5,04
density 156,5 kg/m3)
PAROC ROB60 (t) (20-30 mm thickness, lambda 0,038,
Roofs 1 m2 5,73
average density 173 kg/m3)
PAROC ROB80 (t) (20-30 mm thickness, lambda 0,038,
Roofs 1 m2 6,16
average density 186 kg/m3)
PAROC ROB100 (30-50 mm thickness, lambda 0,039, average
Roofs 1 m2 6,40
density 188,5 kg/m3)
EPD for the best environmental decision 7
PAROC SSB1 (20-50 mm thickness, lambda 0,035, average
Special Applications 1 m2 3,58
density 117,5 kg/m3)
PAROC SSB2 (t) (30 mm thickness, lambda 0,037, average
Special Applications 1 m2 5,40
density 167,5 kg/m3)
PAROC FPS14 (30-100 mm thickness, lambda 0,037, average
Special Applications 1 m2 4,45
density 138 kg/m3)
PAROC FPS17 (20-50 mm thickness, lambda 0,038, average
Special Applications 1 m2 5,63
density 170 kg/m3)
PAROC CGL 20 cy (50-400 mm thickness, lambda 0,037,
Special Applications 1 m2 1,93
average density 60 kg/m3)
PAROC GRS 20 (40-200 mm thickness, lambda 0,035, average
Special Applications 1 m2 2,94
density 96,5 kg/m3)
PAROC COS 5 (40-200 mm thickness, lambda 0,035, average
Facade 1 m2 1,83
density 60 kg/m3)
PAROC WAS 25 (t) (tb) (30-50 mm thickness, lambda 0,033,
Facade 1 m2 2,53
average density 88 kg/m3)
PAROC WAS 35 (t) (tb) (30-200 mm thickness, lambda 0,033,
Facade 1 m2 2,01
average density 70 kg/m3)
PAROC WAS 50 (t) (tb) (50-200 mm thickness, lambda 0,034,
Facade 1 m2 1,33
average density 45 kg/m3)
PAROC WAB 10t (20 mm thickness, lambda 0,036, average
Facade 1 m2 4,70
density 150 kg/m3)
PAROC Linio 10 (cc) (50-200 mm thickness, lambda 0,036,
Facade 1 m2 2,56
average density 81,5 kg/m3)
PAROC Linio 15 (50-180 mm thickness, lambda 0,037,
Facade 1 m2 3,24
average density 100,5 kg/m3)
PAROC Linio 15 (30 mm thickness, lambda 0,037, average
Facade 1 m2 4,03
density 125 kg/m3)
PAROC Linio 15 (30 mm thickness, lambda 0,037, average
Facade 1 m2 4,03
density 125 kg/m3)
PAROC Linio 80 (50-340 mm thickness, lambda 0,040,
Facade 1 m2 2,72
average density 78 kg/m3)
PAROC Linio Pro (50-240 mm thickness, lambda 0,034,
Facade 1 m2 2,55
average density 86 kg/m3)
PAROC Tento (t) (tb) (45-250 mm thickness, lambda 0,033,
Facade 1 m2 2,01
average density 70 kg/ m3)
PAROC Tento (t) (tb) (30 mm thickness, lambda 0,033,
Facade 1 m2 2,30
average density 80 kg/ m3)
EPD for the best environmental decision 8
LCA: Results
The system boundary of the EPD follows the modular structure defined by EN15804+A2. The
table identifies the modules included in this study. The use stage (B1-B7) relating to the
building site is not included in this study, as there are no activites and no significant
environmental impact in the use stage.
System boundaries (X=included, MND= module not declared, MNR=module not
relevant)
Benefits
& loads
Assembly
Product stage Use stage End of life stage beyond
stage
system
boundary
n -
s la ir e t a m w a R t r o p s n a r T g n ir u t c a fu n a M t r o p s n a r T y lb m e s s A e s U e c n a n e t n ia M r ia p e R t n e m e c a lp e R t n e m h s ib r u fe R e s u y g r e n e la n o it a r e p O e s u r e t a w la n o it a r e p O o it ilo m e d n o it c u r t s n eo c - t r o p s n a r T g n is s e c o r p e t s a W la s o p s iD g yn r eil v ec soy uc c ee e RR --la it n e t o p
D R
A1 A2 A3 A4 A5 B1 B2 B3 B4 B5 B6 B7 C1 C2 C3 C4 D
X X X X X MNR MNR MNR MNR MNR MNR MNR X X X X X
Core environmental impact indicators
Indicator Unit A1-A3 A4 A5 C1 C2 C3 C4 D
kg CO2
GWP-total 1,31E+00 2,97E-03 1,70E-01 1,19E-02 3,60E-03 0 1,55E-02 -5,85E-02
eq.
kg CO2
GWP-fossil 1,40E+00 2,93E-03 7,39E-02 1,18E-02 3,56E-03 0 1,54E-02 -5,82E-02
eq.
GWP- kg CO2
-9,44E-02 0 9,60E-02 1,06E-04 2,26E-05 0 5,97E-05 -2,98E-04
biogenic eq.
GWP- kg CO2
2,67E-04 1,64E-05 6,29E-06 2,49E-06 1,97E-05 0 2,85E-05 -6,41E-06
LULUC eq.
kg
ODP CFC11 8,82E-13 1,77E-16 2,81E-14 1,72E-13 2,11E-16 0 3,62E-14 -3,94E-13
eq.
mol H⁺
AP 3,05E-03 2,46E-06 8,25E-05 2,58E-05 1,20E-05 0 1,09E-04 -7,66E-05
eq.
EP-
kg P eq. 7,86E-07 8,80E-09 1,80E-08 3,43E-08 1,05E-08 0 2,61E-08 -8,02E-08
freshwater
EP-marine kg N eq. 6,73E-04 7,03E-07 1,98E-05 5,79E-06 5,58E-06 0 2,80E-05 -2,08E-05
EP- mol N
1,19E-02 8,54E-06 3,36E-04 6,08E-05 6,23E-05 0 3,07E-04 -2,22E-04
terrestial eq.
kg
POCP NMVOC 1,75E-03 2,12E-06 5,17E-05 1,57E-05 1,08E-05 0 8,49E-05 -5,81E-05
eq.
kg Sb
ADP-M&M 6,76E-08 2,46E-10 1,55E-09 3,20E-09 2,95E-10 0 1,58E-09 -8,79E-09
eq.
ADP-fossil MJ 1,32E+01 3,94E-02 2,76E-01 2,13E-01 4,71E-02 0 2,02E-01 -9,89E-01
WDP m³ 3,71E-02 2,64E-05 1,68E-02 2,68E-03 3,16E-05 0 1,69E-03 -6,21E-03
GWP-total: Global Warming Potential; GWP-fossil: Global Warming Potential fossil fuels; GWP-biogenic:
Global Warming Potential biogenic; GWP-LULUC: Global Warming Potential land use and land use change;
EPD for the best environmental decision 9
ODP: Depletion potential of the stratospheric ozone layer; AP: Acidification potential, Accumulated
Exceedance; EP-freshwater: Eutrophication potential, fraction of nutrients reaching freshwater end
compartment; See “additional requirements” for indicator given as PO4 eq. EP-marine: Eutrophication
potential, fraction of nutrients reaching freshwater end compartment; EP-terrestrial: Eutrophication
potential, Accumulated Exceedance; POCP: Formation potential of tropospheric ozone; ADP-M&M: Abiotic
depletion potential for non-fossil resources (minerals and metals); ADP-fossil: Abiotic depletion potential
for fossil resources; WDP: Water deprivation potential, deprivation weighted water consumption
Reading example: 9,0 E-03 = 9,0*10-3 = 0,009
Additional environmental impact indicators
Indicator Unit A1-A3 A4 A5 C1 C2 C3 C4 D
Disease
PM 1,61E-07 2,49E-11 3,10E-09 2,14E-10 6,36E-11 0 1,61E-07 2,49E-11
incidence
IRP kBq U235 eq. 3,24E-02 7,13E-06 9,81E-04 5,78E-03 8,53E-06 0 0,032444 7,13E-06
ETP-fw CTUe 2,93E+00 2,73E-02 6,34E-02 9,35E-02 3,27E-02 0 2,934068 0,027343
HTP-c CTUh 5,68E-10 5,51E-13 1,24E-11 2,68E-12 6,59E-13 0 5,68E-10 5,51E-13
HTP-nc CTUh 5,23E-09 3,04E-11 1,66E-10 9,89E-11 3,95E-11 0 5,23E-09 3,04E-11
SQP Dimensionless 1,59E+01 1,36E-02 4,25E-02 7,69E-02 1,62E-02 0 15,89637 0,013553
PM: Particulate matter emissions; IRP: Ionising radiation, human health; ETP-fw: Ecotoxicity (freshwater);
ETP-c: Human toxicity, cancer effects; HTP-nc: Human toxicity, non-cancer effects; SQP: Land use related
impacts / soil quality
Reading example: 9,0 E-03 = 9,0*10-3 = 0,009
Classification of disclaimers to the declaration of core and additional environmental
impact indicators
ILCD
Indicator Disclaimer
classification
Global warming potential (GWP) None
ILCD type / level
Depletion potential of the stratospheric ozone layer (ODP) None
1
Potential incidence of disease due to PM emissions (PM) None
Acidification potential, Accumulated Exceedance (AP) None
Eutrophication potential, Fraction of nutrients reaching marine end
None
compartment (EP-marine)
ILCD type / level
Eutrophication potential, Accumulated Exceedance (EP-terrestrial) None
2
Formation potential of tropospheric ozone (POCP) None
Potential Human exposure efficiency relative to U235 (IRP) 1
Abiotic depletion potential for non-fossil resources (ADP-minerals&metals) 2
Abiotic depletion potential for fossil resources (ADP-fossil) 2
Water (user) deprivation potential, deprivation-weighted water consumption
2
(WDP)
ILCD type / level
Potential Comparative Toxic Unit for ecosystems (ETP-fw) 2
3
Potential Comparative Toxic Unit for humans (HTP-c) 2
Potential Comparative Toxic Unit for humans (HTP-nc) 2
Potential Soil quality index (SQP) 2
EPD for the best environmental decision 10
Disclaimer 1 – This impact category deals mainly with the eventual impact of low dose ionizing radiation on
human health of the nuclear fuel cycle. It does not consider effects due to
possible nuclear accidents, occupational exposure nor due to radioactive waste disposal in underground facilities.
Potential ionizing radiation from the soil, from radon and from some
construction materials is also not measured by this indicator.
Disclaimer 2 – The results of this environmental impact indicator shall be used with care as the uncertainties on
these results are high or as there is limited experienced with the indicator
Resource use
Parameter Unit A1-A3 A4 A5 C1 C2 C3 C4 D
RPEE MJ 1,51E+00 2,24E-03 1,09E+00 1,18E-01 2,68E-03 0 6,65E-02 -2,72E-01
RPEM MJ 1,09E+00 0 -1,06E+00 0 0 0 -3,62E-02 0
TPE MJ 2,60E+00 2,24E-03 3,72E-02 1,18E-01 2,68E-03 0 3,03E-02 -2,72E-01
NRPE MJ 1,12E+01 3,95E-02 8,51E-01 2,13E-01 4,72E-02 0 1,60E+00 -9,90E-01
NRPM MJ 1,97E+00 0 -5,74E-01 0 0 0 -1,39E+00 0
TRPE MJ 1,32E+01 3,95E-02 2,77E-01 2,13E-01 4,72E-02 0 2,02E-01 -9,90E-01
SM kg 1,94E-01 0 3,88E-03 0 0 0 0 0
RSF MJ 0 0 0 0 0 0 0 0
NRSF MJ 0 0 0 0 0 0 0 0
W m3 2,34E-03 2,53E-06 4,24E-04 1,13E-04 3,03E-06 0 5,13E-05 -2,62E-04
RPEE Renewable primary energy resources used as energy carrier; RPEM Renewable primary energy
resources used as raw materials; TPE Total use of renewable primary energy resources; NRPE Non-
renewable primary energy resources used as energy carrier; NRPM Non-renewable primary energy
resources used as materials; TRPE Total use of non-renewable primary energy resources; SM Use of
secondary materials; RSF Use of renewable secondary fuels; NRSF Use of non-renewable secondary fuels; W
Use of net fresh water
Reading example: 9,0 E-03 = 9,0*10-3 = 0,009
End of life - Waste
Parameter Unit A1-A3 A4 A5 C1 C2 C3 C4 D
HW kg 4,91E-07 1,89E-13 9,82E-09 1,85E-11 2,26E-13 0 1,04E-11 -1,34E-10
NHW kg 1,24E-01 5,66E-06 2,42E-02 1,61E-04 6,77E-06 0 1,03E+00 -5,00E-04
RW kg 2,85E-04 4,86E-08 7,67E-06 3,41E-05 5,82E-08 0 2,25E-06 -7,81E-05
HW Hazardous waste disposed; NHW Non-hazardous waste disposed; RW Radioactive waste disposed
Reading example: 9,0 E-03 = 9,0*10-3 = 0,009
End of life – output flow
Parameter Unit A1-A3 A4 A5 C1 C2 C3 C4 D
CR kg 0 0 0 0 0 0 0 0
MR kg 0 0 0 0 0 0 0 0
MER kg 0 0 7,82E-02 0 0 0 0 0
EEE MJ 0 0 0 0 0 0 0 0
ETE MJ 0 0 0 0 0 0 0 0
EPD for the best environmental decision 11
CR Components for reuse; MR Materials for recycling; MER Materials for energy recovery; EEE Exported
electric energy; ETE Exported thermal energy
Reading example: 9,0 E-03 = 9,0*10-3 = 0,009
Information describing the biogenic carbon content at the factory gate
Biogenic carbon content Unit Value
Biogenic carbon content in product kg C 0
Biogenic carbon content in the accompanying packaging kg C 1,02E+00
EPD for the best environmental decision 12
Additional requirements
Greenhous gas emission from the use of electricity in the manufacturing phase
National production mix from import, low voltage (production of transmission lines, in addition
to direct emissions and losses in grid) of applied electricity for the manufacturing process (A3).
National electricity grid Unit Value
Electricity, grid mix, Lithuania kg CO2 -eq/kWh 4,12E-01
Additional environmental impact indicators required in NPCR Part A for construction
products
In order to increase the transparency of biogenic carbon contribution to climate impact, the
indicator GWP-IOBC is required as it declares climate impacts calculated according to the
principle of instantaneous oxidation. GWP-IOBC is also referred to as GWP-GHG in context to
Swedish public procurement legislation.
Indicator Unit A1-A3 A4 A5 C1 C2 C3 C4 D
kg CO2
GWP-IOBC 1,40E+00 2,94E-03 7,39E-02 1,18E-02 3,58E-03 0 1,54E-02 -5,82E-02
eq.
GWP-IOBC Global warming potential calculated according to the principle of instantaneous oxidation.
Hazardous substances
The declaration is based upon reference to threshold values and/or test results and/or material
safety data sheets provided to EPD verifiers. Documentation available upon request to EPD
owner.
x□ The product contains no substances given by the REACH Candidate list or the
Norwegian priority list.
□ The product contains substances given by the REACH Candidate list or the Norwegian
priority list that are less than 0,1 % by weight.
□ The product contains dangerous substances, more then 0,1% by weight, given by the
REACH Candidate List or the Norwegian Priority list, see table.
□ The product contains no substances given by the REACH Candidate list or the
Norwegian priority list. The product is classified as hazardous waste (Avfallsforskiften,
Annex III), see table.
Indoor environment
The products covered by this EPD meet the legal requirements for stone wool thermal
insulation.
Carbon footprint
Carbon footprint has not been worked out for the product.
EPD for the best environmental decision 13
Bibliography
ISO 14025:2010 Environmental labels and declarations - Type III environmental declarations -
Principles and procedures
ISO 14044:2006 Environmental management - Life cycle assessment - Requirements and
guidelines
ISO 21930:2007 Sustainability in building construction - Environmental declaration of building
products
ISO 14040 EN ISO 14040:2009-11 Environmental management - Life cycle assessment -
Principles and framework
EN 15804:2012+A2:2019 Sustainability of construction works - Environmental product declaration - Core
rules for the product category of construction products
EN 12939:2000 Thermal performance of building materials and products – Determination of
thermal resistance by means of guarded hot plate and heat flow meter methods
– Products oh high and medium thermal resistance
EN 12667:2001 Thermal performance of building materials and products – determination of
thermal resistace by means of guarded hot plate and heat flow meter methods –
products of high and medium thermal resistance
EN 13501-1:2007+A1:2009 Fire classification of construction products and building elements – part 1:
Classification using data from reaction to fire tests
PCR NPCR PART A Construction Products and Services
PCR NPCR 012 Part B for Thermal Insulation Products.
CPR Regulation (EU) No 305/2011 of the European parliament and of the council of
9 March 2011 laying down harmonised conditions for the marketing of
construction products and repealing Council Directive 89/106/EEC
CEN/TR 15941 Sustainability of construction works – Environmental product declarations –
Methodology for selection and use of generic data; CEN/TR 15941:2010
DYNEA 2022 LCA results for 3 different binder data, results according EN 15884+A2, 2022
GaBi ts GaBi ts dataset documentation for the software-system and databases, LBP,
University of Stuttgart and Sphera, Leinfelden-Echterdingen, 2022
(https://www.gabi-software.com/support/gabi)
GHG 2022 Greenhouse gas conversion factors,
https://www.gov.uk/government/publications/greenhouse-gas-reporting-
conversion-factors-2022
Singh P, Goymann M, Goerke J Background report for EPD of Paroc Stone Wool Insulation, January 2023.
Program Operator tlf +47 23 08 80 00
The Norwegian EPD Foundation
Post Box 5250 Majorstuen, e-
post@epd-norge.no
0303 Oslo post:
Norway web www.epd-norge.no
Publisher tlf +47 23 08 80 00
The Norwegian EPD Foundation
Post Box 5250 Majorstuen, e-
post@epd-norge.no
0303 Oslo post:
Norway web www.epd-norge.no
Owner of the declaration tlf +358 46 876 8000
Company Logo Paroc Group Oy e- InsulationEurope.Sustainability@owenscorning.com
post:
FI-00181, Helsinki, Finland web www.paroc.com
Author of the life cycle
tlf +49 711 34 18 17-25
assessment
Company Logo
e-
Sphera Solutions GmbH info@sphera.com
post:
Singh P, Goymann M, Goerke J web www.sphera.com
ECO Platform web www.eco-platform.org
ECO Portal web ECO Portal
EPD for the best environmental decision 14
EPD for the best
environmental
decision
The Norwegian EPD foundation
www.epd-norge.no
EPD for the best environmental decision 15
