Environmental Product
Declaration
as per ISO 14025 and EN 15804+A2
Owner of the declaration: AS BMGS
Publisher: Kiwa-Ecobility Experts
Program operator: Kiwa-Ecobility Experts
Registration number: EPD-BMGS-312-EN
Issue date: 23.08.2023
Valid to: 23.08.2028
Structural stairs and landings
1. General information
AS BMGS Precast concrete elements
Programme operator Owner of the declaration
Kiwa-Ecobility Experts AS BMGS
Kiwa GmbH Tvaika iela 27
Voltastr. 5 LV-1005 Riga
13355 Berlin Latvia
Germany
Registration number Declared product / declared unit
EPD-BMGS-312-EN 1 ton of a precast concrete element
This declaration is based on the Product Scope
Category Rules The EPD (type: Cradle to gate with options,
EN 16757:2022 Sustainability of construction modules C1-C4 and module D (A1-A5, C, D) is
works – Environmental product declarations about custom made precast concrete
– Product Category Rules for concrete and elements – stairs and landings, manufactured
concrete elements in Riga, Latvia. The calculation is based on 1
metric ton of a precast concrete element with
Issue date
a share of 3,05m% reinforcing steel.
23.08.2023
Kiwa-Ecobility Experts shall not be liable with
Valid to respect to manufacturer information, life
23.08.2028 cycle assessment data and evidence.
Verification
The standard EN 15804+A2:2019 serves as the
core PCR
Independent verification of the declaration
and data according to ISO 14025:2006
☐internal ☒external
Frank Huppertz
(Head of Kiwa-Ecobility Experts)
Prof. Dr. Frank Heimbecher Elisabet Amat Guasch
(Chairman of the independent expert committee – (External verifier)
Ecobility Experts)
Page | 2 AS BMGS – Structural stairs and landings
2. Product
2.1 Product description
The products – structural stairs and landings – are precast concrete elements in which the reinforcing
steel constitutes the main reinforcement of the composite slab. The products are produced in various
sizes and shapes with concrete compressive strength class of C30/37 to C40/50 (normative minimum
concrete compressive strength class is C25/30).
2.2 Application
The precast concrete stairs and associated landings are intended to be used as the structural system
of a building or other structures (including industrial and storage buildings, public buildings etc.).
2.3 Placing on the market / Application rules
The harmonized standard EN 13369 (Common rules for precast concrete products) together with
supplementary Swedish requirements and product-specific standard EN 14843 (Precast concrete
products - Stairs) apply for the production of the products. The CE mark is applied to the finished
products. Producer is authorized to use Nordcerts registered BBC mark.
Additional certifications: the production of AS BMGS of precast concrete elements is certified in
accordance with the requirements of management system standards ISO 9001:2015, ISO 14001:2015,
ISO 45001:2018, ISO 50001:2018.
Market: Scandinavian countries – Sweden, Norway, Denmark and Finland. The Swedish market is used
for modelling A4-A5 and C1-C4.
2.4 Technical Data
Technical Data – Precast concrete stairs
Name Value Unit
Compressive strength C30/37 – C40/50 N/mm2
Reinforcing steel B500B B500C -
Ultimate tensile strength Re 500 500 N/mm2
Tensile yield strength Rm 540 575-675 N/mm2
Durability of product 50 years
Tolerances Svensk Betong "Toleranser för betongelement" 2020 Class А; B
Length – up to 10 m, width – up to 4 m, height – up to 1,5 m. Average weight around 10 t.
2. 5 Base materials / Ancillary
Name Value Unit
Cement 13,47 m%
Aggregates 77,26 m%
Water 6,14 m%
Admixture 0,08 m%
Steel* 3,05 m%
*Post-consumer recycled content 29,55% (based on the documentation of the background process).
Neither the product itself nor the packaging contains biogenic carbon, so the biogenic carbon content
at the factory gate is 0 kg.
2.5 Manufacturing
The manufacturing contains the following processes:
• Delivery of raw materials;
Page | 3 AS BMGS – Structural stairs and landings
• Preparation of the molds (plywood formwork, cutting and laying of the probation steel
elements, placeholders etc.);
• Concrete mixing and filling into the molds, curing;
• Removal of the formwork, finishing, storage.
Figure 1: Overview of the production route of a precast concrete element (A1-A5, C1-C4, D)
2.6 Packaging
The only packaging is wood spacers and since they are re-used, they fall under cut-off rules and
therefore are not included in the LCA calculations. The transportation does not cause any losses as
products are secured properly.
2.7 Production waste
The data on generated production waste is recorded as accurately as possible. Thus, the generated
production waste is allocated per declared unit. No loses for cement are assumed since filters are used
to collect dust in the air of cement storage in silos. The captured cement dust is reused in production.
No loses for inert materials are assumed too since materials are stored in open warehouses, which
three sides are enclosed by a wall. The same assumptions are made for other components. There is no
production waste for scrap metal, because reinforcement steel is delivered of the size as in the
drawings (no cutting is made).
Page | 4 AS BMGS – Structural stairs and landings
3. LCA: Calculation rules
3.1 Declared unit
The EPD refers to the declared product system of 1 metric ton of precast concrete element.
Name Value Unit
Declared unit 1 ton
Cement type* CEM II/A-M(S-LL) 52,5N -
Compressive strength class** C30/37 – C40/50 -
Percentage of reinforcing steel 3,05 m%
Steel grade B500B / B500C -
* CEM II/A-M(S-LL) 52,5N is used for LCA calculations (data from specific EPD).
** Concrete mixes are produced according to recipes, in compliance with the strictest quality norms and
standards in force, as well as the specific purposes for which a particular batch of concrete is intended.
3.2 System boundary
This EPD was created in accordance with EN 15804 requirements and includes the production stage,
transportation to the site, construction process and the end-of-life stage. According to EN 15804 this
corresponds to product phases A1-A5, C1-C4 and D (EPD type "Cradle to gate with options, modules
C1-C4 and module D" (A1-A3, C, D and additional modules A4 and A5)).
The production process of a precast concrete element begins with the preparation of molds. This
includes assembly of the molds depending on the dimensions of the element, cleaning of the molds
and application of mold oil (release agent). After that, the reinforcing steel parts are placed according
to the technical drawing of the element. Wet concrete (site-mixed) is then poured into the molds and
vibrated into place, and the surface is treated. After casting, the element is covered and cured. After
curing, it is removed from the mold and taken out of the factory. Eventually, it is transported to the
construction site.
Production stage
A1: This stage considers the extraction and processing of raw materials as well as energy consumption.
All installed raw materials of the products were analyzed, and the masses were determined.
A2: The raw materials are transported to the production plant. In this case, the model includes road or
road and maritime transportation of each raw material. Supplier information regarding the transport
distances and vehicle type were provided by AS BMGS or chosen from relevant market profiles. Where
no precise information on secondary materials, secondary fuels and waste is not available, secondary
content is indicated based on the documentation of the background processes.
A3: This stage includes the manufacture of products. It also considers the energy consumption and
waste generated at the production plant. The processes that are considered at the production site are:
preparation of the molds (OSB formwork, cutting and laying of the probation steel elements,
placeholders); concrete mixing and filling into the molds, curing; removal of the formwork, finishing,
and storage. The national electricity mix of Latvia was taken into account.
Assembly stage
A4: This stage includes transport from the production stockyard to the construction site where the
prefabricated product shall be installed.
A5: Installation is modelled as assembly of a typical concrete product in a building. Fossil fuel for lifting
machinery and ancillary materials are included.
Page | 5 AS BMGS – Structural stairs and landings
Use stage
B1 to B7: The use of the final product is not within the manufacturer's sphere of influence. Therefore,
modules B1-7 have not been considered.
End of life stage
C1: Deconstruction module concerns the deconstruction of the concrete element, whereby no
environmental impact (emissions to air, soil or water) was assumed. According to the current state of
the art, the demolition of concrete and reinforced concrete structures is mainly carried out with
longfront excavators equipped with demolition clamps.
C2: Transport module concerns transportation to waste processing. All of end-of-life product is
assumed to be sent to the closest facilities (C2).
Transport to waste processing (C2)
Name Vehicle type Distance
Truck* Lorry (Truck), unspecified (default) | market group Landfill:100 km; Incineration: 150
for (GLO) km (energy recovery on site 0);
Recycling: 50 km; Re-Use: 0 km
* For all transports, the environmental profile of a non-specific truck transport was used (conservative
assumption): The vehicle operates with diesel, and it provides a fleet average that includes different lorry classes
as well as EURO classes. This transport used an average load factor, including empty return trips.
C3 and C4: At the end-of-life, in the demolition phase 100% of a concrete element is assumed to be
collected as separate construction waste. The waste is assigned to the material-specific disposal route
(C3) – waste processing (for reuse, recovery and/or recycling) or (C4) - landfill.
End of life (C1-C4)
Name Value Unit
Collected separately waste type 1000 kg
Collected as mixed construction waste 0,00 kg
Re-use 0,00 kg
Recycle 988,78 kg
Energy recovery 0,00 kg
Landfilling 11,22 kg
D: The benefits beyond life cycle has been modelled based on the output flows from module C3. This
includes materials recovered from the waste flow.
All inputs including raw materials, primary products, energy and auxiliary materials as well as the
accumulated waste are considered in the assessment. The use of the final product is not within the
manufacturer's sphere of influence. Therefore, modules B1-7 have not been considered. The effect of
CO absorption through the carbonization process is not taken into account in the LCA. The reference
2
year to collect all input data is 2022. The geographical reference area is Europe or Global and can be
seen in the system description boundary table.
3.3 Estimates and assumptions
All installed raw materials of the products were analyzed, and the masses were determined following
the allocation and cut-off requirements. Production-specific energy consumption were measured and
provided by AS BMGS. Supplier information regarding the transport distances were provided by AS
BMGS. The raw material data for each of the product produced is recorded to a high standard of
accuracy and precision. The energy consumption, ancillary materials and production waste is allocated
according to the annual production of the declared unit to the total annual production at the factory.
Page | 6 AS BMGS – Structural stairs and landings
3.4 Cut-off criteria
The study does not exclude any modules or processes which are stated mandatory in the EN 15804
and applicable PCR. The study does not exclude any hazardous materials or substances included in the
Candidate List of Substances of Very High Concern (SVHCs) for authorization with concentrations
higher than 0.1% weight by weight. All material flows that contribute to more than 1% of the total
mass, energy or environmental impact of the system have been considered in the LCA. It can be
assumed that the neglected processes in total contributed less than 5% to the considered impact
categories.
The product stage includes materials, energy and waste flows only related to production processes
(e.g. energy and water use related to company management and sales activities are excluded where
technically possible; production, manufacture, and construction of manufacturing capital goods and
infrastructure, other processes which are not directly related to the production of concrete elements).
3.5 Background Data
The Life Cycle Assessment was modelled with the R<THiNK software from NIBE. The background data
is taken from Ecoinvent version 3.6 (2019) “Allocation, cut-off” database. Geographical reference
space of the background data is Europe or Global. Almost all consistent datasets contained in the
Ecoinvent database are documented and can be viewed in the online Ecoinvent documentation. The
reference year to collect all input data is 2022. The geographical reference area is Europe or Global
and can be seen in the system description boundary table.
3.6 Data quality
In the operating data survey all relevant process-specific data has been collected. The data relating to
the manufacturing phase of the precast concrete element was determined by AS BMGS and refers to
production site in Riga, Tvaika street 27. The data relating to the manufacturing construction phase
are determined also by BMGS and refers to the finished construction project in Sweden.
Secondary data was taken from the Ecoinvent 3.6 (2019) database. The database is regularly checked
and thus complies with the requirements of ISO 14040/44 (background data not older than 10 years).
The background data meets the requirements of EN 15804.
The general rule was followed that specific data from specific production processes or average data
derived from specific processes must be given priority when calculating an EPD or Life Cycle
Assessment. Data for processes that the manufacturer cannot influence or choose, were backed up
with generic data.
3.7 Period Under review
All process-specific data was collected for the manufacturing year 2022. The quantities of raw and
ancillary materials as well as energy consumption have been recorded and averaged over the entire
operating year 2022.
3.8 Allocation
There are no co-products in the raw material supply phase, so no allocation methods were used at this
stage. There are no allocations during the manufacturing phase at the plant. Appropriation or
attribution of inputs and outputs, e.g. auxiliary materials, energy (utilities), waste has been done on
the basis of production volumes in 2022 (reference year).
The background data is taken from Ecoinvent version 3.6 (2019) Allocation, cut-off library. Almost all
consistent datasets contained in the Ecoinvent database is documented and can be viewed in the
online Ecoinvent documentation. Allocation principles in the background are in compliance with the
Page | 7 AS BMGS – Structural stairs and landings
foreground. Specific information on allocations within the background data can be found in the
Ecoinvent database version 3.6 (2019) document.
3.9 Calculation methods
For life cycle assessment, the calculation methods described in ISO 14040 have been applied. The
evaluation is based on the phases in the system boundaries.
3.10 Mix of electricity and CO -Certificates
2
The electricity mix (medium voltage) was chosen, using the country-specific market dataset (Latvia)
from the background database. Reference year of the dataset 2019, reference year of the electricity
mix is at least 2012. The Ecoinvent profile used for the gridmix includes the imported energy and
excludes the exported energy.
3.11 Comparability
EPD of construction products may not be comparable if they do not comply with the requirements of
EN 15804. Basically, a comparison or an evaluation of EPD data is only possible if all the data sets to be
compared were created according to EN 15804 and the building context, respectively the product-
specific characteristics of performance, are considered.
3.12 Reference Service Life (RSL)
The concrete composition limits given in EN 206 are specified for an intended service life of at least 50
years under the respective exposure classes/ environmental conditions.
Page | 8 AS BMGS – Structural stairs and landings
4. LCA: Scenarios and additional technical information
Module A4: This stage includes transport from the production stockyard to the construction site where
the prefabricated product shall be installed. Basic scenario transportation from AS BMGS production
site in Latvia to customer in Sweden, Stockholm, with distance radius around 100 km. Transportation
is calculated based on data form manufacturer and the scenario with the parameters described in the
following table. The transportation does not cause losses as products are secured properly.
Transport from production place to the construction site (A4)
Parameter Vehicle type Distance
Truck* Lorry >32t, EURO5 280 km**
Maritime Ferry/ Transoceanic freight ship, containers 270 km
* Data for transport is calculated for an average load factor, including empty return trips
** Total distance by truck: from Riga factory to the port located in Ventspils city (180 km) and from the port in
Sweden to the construction site (100 km)
Module A5: Installation is modelled as assembly of a typical concrete product in a building. Fossil fuel
for lifting machinery and ancillary materials are included.
Mostly the erection of the elements is performed directly from the trailers without putting them in a
temporary storage at the construction site. It is assumed that there is negligible waste during assembly.
The energy required for the installation process as well as the ancillary materials are calculated based
on the data, which comes from the KVINSTA project implemented in 2020. The values for the precast
element assembly process are provided by AS BMGS.
Assembly (A5)
Name Value Unit
Auxiliary* 15,0 kg
Water consumption 2,1 kg
Fuel 1,44 l
* Auxiliary material cement is included.
Modules B1 to B7: For concrete components, maintenance and repair measures are generally not
necessary during the reference service life, so that no environmental burdens arise in these modules.
In addition, no energy or water is consumed.
C1 Demolition: Based on Bozdağ, Ö., Seçer, M. (2007) energy consumption of a demolition process is
on the average 10 kWh/m2 and an average mass of a reinforced concrete building is about 1000 kg/m2.
Therefore, energy consumption demolition is 10 kWh/1000 kg. The source of energy is diesel fuel used
by work machines and based on the statements above can be assumed being 1,009 l (with NCV
42,49 GJ/t).
C2 – C4 and D: It is assumed that concrete and reinforcement material are separated after
deconstruction. For the both waste groups, waste scenarios according to the Dutch National
Environmental Database NMD (2022) is applied:
• Concrete (i.a. elements, brickwork, reinforced concrete): 99% of concrete is recycled and then
reused as aggregate.
• Steel, reinforcement: 95% of reinforcing steel is marketed as scrap metal.
The effect of CO2 absorption through the carbonization process in the use and end-of-life phase is not
assessed here and taken into account in the LCA. According to the PCR for concrete and concrete
elements (EN 16757), carbonation is not mandatory to be reported.
Page | 9 AS BMGS – Structural stairs and landings
5. LCA: Results
This Life cycle assessment is made for EPD type “Cradle to gate with options, modules C1-C4 and
module D”. The Environmental Product Declaration analyses the Production stage (A1-A3), the
Construction process stage (A4-A5), the End-of-life stage (C1-C4) and the Benefits and loads beyond
the system boundary (D).
Description of the system boundary
Benefits and
Construction loads beyond
Product stage Use stage End of life stage
process stage the system
boundaries
y lp p u s la ir e t a m w a R t r o p s n a r T g n ir u t c a fu n a M u n a m m o r f t r o p s n a r T-e s u fo re ec ra ulp t c o at f n on io t cit ua rl tl sa nts on C-is s e c o r p e s U e c n a n e tn ia M r ia p e R tn e m e c a lp e R tn e m h s ib r u fe R e s u y g r e n e la n o it a r e p O e s u r e t a w la n o it a r e p O / n o it c u r ts n eo Dc -n o itilo m e d t r o p s n a r T g n is s e c o r p e ts a W la s o p s iD y r e v eo s uc ee RR -- gla ni it ln c ye ct o e Rp -
A1 A2 A3 A4 A5 B1 B2 B3 B4 B5 B6 B7 C1 C2 C3 C4 D
X X X X X MND MND MND MND MND MND MND X X X X X
Geography
EU EU LV EU EU MND MND MND MND MND MND MND EU EU EU EU EU
X=Module declared | MND=Module not declared
All major materials, production energy use and waste are included for phases A1, A2, A3, A4, A5, C1,
C2, C3 and C4. Use stage B1-B7 is not relevant for this type of product and is not declared.
The following tables show the results of the impact assessment indicators, resource use, waste and
other output streams. The results presented here refer to the declared average product.
Disclaimer on ADP-e, ADP-f, WDP, ETP-fw, HTP-c, HTP-nc, SQP: The results of these environmental
impact indicators must be used with caution, as the uncertainties in these results are high or as there
is limited experience with the indicator.
Disclaimer on IR: This impact category mainly addresses the potential effect of low dose ionizing
radiation on human health in the nuclear fuel cycle. It does not consider effects due to possible nuclear
accidents and occupational exposures, nor does it consider radioactive waste disposal in underground
facilities. Potential ionizing radiation from soil, radon, and some building materials is also not measured
by this indicator.
Page | 10 AS BMGS – Structural stairs and landings
Results of the LCA – Environmental impact: 1 metric t of precast concrete structural stairs
Parameter Unit A1 A2 A3 A4 A5 C1 C2 C3 C4 D
Core environmental impact indicators (EN 15804)
ADP-f MJ 9,46E+02 1,64E+02 1,75E+02 4,28E+02 1,25E+02 4,55E+01 1,03E+02 4,48E+01 1,65E+00 -2,49E+02
ADP-mm kg Sb-eqv. 1,12E-03 2,79E-04 8,98E-05 4,53E-04 5,18E-05 5,07E-06 1,73E-04 7,30E-06 5,41E-07 -2,23E-04
AP mol H+ eqv. 5,47E-01 5,36E-02 3,78E-02 1,90E-01 8,18E-02 3,46E-02 3,96E-02 2,74E-02 5,61E-04 -1,39E-01
EP-fw kg P eqv. 3,68E-03 8,50E-05 2,57E-04 2,04E-04 1,66E-04 1,20E-05 6,88E-05 5,96E-05 6,62E-07 -1,15E-03
EP-m kg N eqv. 1,59E-01 1,80E-02 1,22E-02 5,25E-02 3,04E-02 1,53E-02 1,39E-02 1,16E-02 1,93E-04 -2,88E-02
EP-T mol N eqv. 1,75E+00 1,98E-01 1,26E-01 5,82E-01 3,40E-01 1,68E-01 1,54E-01 1,28E-01 2,13E-03 -3,35E-01
GWP-b kg CO2 eqv. 8,90E-02 6,08E-03 2,28E+00 1,77E-02 1,96E-01 9,20E-04 3,15E-03 1,09E-02 1,17E-04 2,77E-01
GWP-f kg CO2 eqv. 1,53E+02 1,08E+01 1,15E+01 2,80E+01 1,75E+01 3,31E+00 6,82E+00 3,27E+00 5,91E-02 -3,25E+01
GWP-luluc kg CO2 eqv. 4,19E-02 3,71E-03 1,14E-02 9,19E-03 2,62E-03 2,61E-04 2,50E-03 5,35E-04 1,65E-05 1,66E-02
GWP-total kg CO2 eqv. 1,53E+02 1,08E+01 1,38E+01 2,80E+01 1,77E+01 3,31E+00 6,83E+00 3,28E+00 5,92E-02 -3,22E+01
ODP kg CFC 11 eqv. 5,86E-06 2,48E-06 1,60E-06 6,49E-06 1,61E-06 7,14E-07 1,51E-06 5,65E-07 2,43E-08 -1,10E-06
POCP kg NMVOC eqv. 5,78E-01 5,74E-02 4,53E-02 1,73E-01 9,17E-02 4,61E-02 4,39E-02 3,50E-02 6,18E-04 -1,89E-01
WDP m3 world eqv. 9,29E+03 4,69E-01 1,24E+02 1,33E+00 1,04E+00 6,10E-02 3,68E-01 1,36E-01 7,40E-02 -6,42E+01
Additional environmental impact indicators (EN 15804)
ETP-fw CTUe 2,37E+03 1,32E+02 1,80E+02 3,36E+02 1,30E+02 2,74E+01 9,18E+01 3,15E+01 1,07E+00 -1,03E+03
HTP-c CTUh 3,90E-07 3,63E-09 3,26E-08 9,21E-09 3,35E-09 9,59E-10 2,98E-09 9,08E-10 2,48E-11 -6,72E-09
HTP-nc CTUh 3,62E-06 1,44E-07 3,06E-07 3,75E-07 1,31E-07 2,36E-08 1,00E-07 2,38E-08 7,61E-10 5,41E-06
IR kBq U235 eqv. 2,49E+00 7,19E-01 3,14E-01 1,87E+00 5,52E-01 1,95E-01 4,31E-01 1,73E-01 6,77E-03 2,79E-01
PM disease incidence 6,95E-06 8,07E-07 3,84E-07 2,38E-06 1,52E-06 9,17E-07 6,14E-07 6,77E-07 1,09E-08 -2,15E-06
SQP Pt 3,96E+02 1,24E+02 1,05E+03 4,58E+02 3,39E+01 5,81E+00 8,92E+01 7,08E+00 3,46E+00 -1,10E+02
ADP-e=Depletion of abiotic resources-elements | ADP-f=Depletion of abiotic resources-fossil fuels | AP=Acidification of soil and water | EP-fw =Eutrophication, freshwater | EP-m=Eutrophication marine |
EP-T=Eutrophication, terrestrial | GWP-b=Global warming potential - Biogenic | GWP-f=Global warming potential - Fossil | GWP-luluc=Global warming potential - Land use and land use change |GWP-total=Global warming
potential |ODP=Ozone layer depletion |POCP=Photochemical oxidants creation | WDP=Water use | ETP-fw=Ecotoxicity, freshwater | HTP-c=Human toxicity, cancer | HTP-nc=Human toxicity, non-cancer | IR=Ionising
radiation, human health | PM=Particulate Matter | SQP=Land use
Page | 11 AS BMGS – Structural stairs and landings
Resource use and environmental information: 1 metric t of precast concrete structural stairs
Parameter Unit A1 A2 A3 A4 A5 C1 C2 C3 C4 D
PERE MJ 9,20E+01 2,29E+00 1,07E+02 5,20E+00 3,57E+00 2,46E-01 1,29E+00 1,50E+00 1,34E-02 2,22E+00
PERM MJ 9,24E-02 0,00E+00 7,51E+01 0,00E+00 0,00E+00 0,00E+00 0,00E+00 0,00E+00 0,00E+00 0,00E+00
PERT MJ 9,21E+01 2,29E+00 1,82E+02 5,20E+00 3,57E+00 2,46E-01 1,29E+00 1,50E+00 1,34E-02 2,22E+00
PENRE MJ 9,85E+02 1,75E+02 1,74E+02 4,55E+02 1,33E+02 4,83E+01 1,09E+02 4,76E+01 1,75E+00 -2,60E+02
PENRM MJ 4,57E+00 0,00E+00 1,62E+01 0,00E+00 0,00E+00 0,00E+00 0,00E+00 0,00E+00 0,00E+00 0,00E+00
PENRT MJ 9,90E+02 1,75E+02 1,90E+02 4,55E+02 1,33E+02 4,83E+01 1,09E+02 4,76E+01 1,75E+00 -2,60E+02
SM Kg 2,02E+01 0,00E+00 3,35E-01 0,00E+00 0,00E+00 0,00E+00 0,00E+00 2,89E+01 0,00E+00 0,00E+00
RSF MJ 5,95E+01 0,00E+00 7,74E-01 0,00E+00 0,00E+00 0,00E+00 0,00E+00 0,00E+00 0,00E+00 0,00E+00
NRSF MJ 2,90E+02 0,00E+00 3,77E+00 0,00E+00 0,00E+00 0,00E+00 0,00E+00 0,00E+00 0,00E+00 0,00E+00
FW m3 1,32E+00 1,75E-02 1,07E-01 4,68E-02 3,51E-02 2,34E-03 1,25E-02 8,98E-03 1,76E-03 -1,48E+00
HWD Kg 2,31E-02 4,26E-04 4,82E-04 9,89E-04 2,41E-04 1,24E-04 2,61E-04 9,94E-05 2,47E-06 -3,51E-03
NHWD kg 1,82E+01 8,76E+00 1,97E+00 3,45E+01 1,44E+00 5,39E-02 6,53E+00 2,95E+00 1,12E+01 -3,33E+00
RWD kg 3,07E-03 1,12E-03 3,91E-04 2,93E-03 7,90E-04 3,16E-04 6,76E-04 2,60E-04 1,08E-05 -5,58E-05
CRU kg 0,00E+00 0,00E+00 0,00E+00 0,00E+00 0,00E+00 0,00E+00 0,00E+00 0,00E+00 0,00E+00 0,00E+00
MFR kg 1,43E-02 0,00E+00 1,17E+01 0,00E+00 1,69E+01 0,00E+00 0,00E+00 9,60E+02 0,00E+00 0,00E+00
MER kg 4,23E-02 0,00E+00 5,50E-04 0,00E+00 0,00E+00 0,00E+00 0,00E+00 0,00E+00 0,00E+00 0,00E+00
EET MJ 2,14E-01 0,00E+00 -2,07E+01 0,00E+00 0,00E+00 0,00E+00 0,00E+00 0,00E+00 0,00E+00 0,00E+00
EEE MJ 1,41E-02 0,00E+00 -1,20E+01 0,00E+00 0,00E+00 0,00E+00 0,00E+00 0,00E+00 0,00E+00 0,00E+00
PERE=renewable primary energy ex. raw materials | PERM=renewable primary energy used as raw materials | PERT=renewable primary energy total | PENRE=non-renewable primary energy ex. raw materials | PENRM=non-
renewable primary energy used as raw materials | PENRT=non-renewable primary energy total | SM=use of secondary material | RSF=use of renewable secondary fuels | NRSF=use of non-renewable secondary fuels |
FW=use of net fresh water | HWD=hazardous waste disposed | NHWD=non-hazardous waste disposed | RWD=radioactive waste disposed | CRU=Components for re-use | MFR=Materials for recycling | MER=Materials
for energy recovery | EET=Exported Energy Thermic | EEE=Exported Energy Electric
Page | 12 AS BMGS – Structural stairs and landings
6. LCA: Interpretation
The following figure shows the influence of the different life stages for the structural stairs. Since the
Global Warming Potential biogen (GWP-b) and Global Warming Potential resulting from land use and
land use change (GWP-luluc) have a minor impact, only the total Global Warming Potential (GWP-total)
is displayed.
Structural stairs
100%
50%
0%
-50%
-100%
A1 A2 A3 A4 A5 C1 C2 C3 C4 D
Figure 2: Influence of the modules on the environmental core indicators
As shown in the figure, the most of the environmental impact is attributed to raw material processing
phase (A1), followed by the transportation of the finished product (A4, Sweden scenario) and
production (A3). Potential credits come mainly from the material recovery of concrete and
reinforcement steel.
Overall, the quality of the data can be considered as good overall. The primary data collection has been
done thoroughly. Data quality was calculated using the Data Quality level and criteria according to the
PEF approach (Annex E.2 of EN15804+A2). The DQRs range from 1,00 to 2,67 for the most abundant
inputs in terms of mass.
Page | 13 AS BMGS – Structural stairs and landings
7. Additional information: Norwegian requirements
Greenhouse gas emissions from the use of electricity mix in the manufacturing phase
Data source Amount Unit
Ecoinvent 3.6 (year 2019) 0,526 CO2-eqv/kWh
Dangerous substances disclaimer
The product contains no substances given by the REACH Candidate list or the Norwegian
☐
priority list
The product contains substances given by the REACH Candidate list or the Norwegian priority
☒
list that are less than 0,1 % by weight.
The product contain dangerous substances, more then 0,1% by weight, given by the REACH
☐
Candidate List or the Norwegian Priority list, see table.
The product contains no substances given by the REACH Candidate list or the Norwegian
☐ priority list. The product is classified as hazardous waste (Avfallsforskiften, Annex III), see
table.
Indoor environment
The EPD does not give information on release of dangerous substances to indoor air because the
horizontal standards on measurement of release of regulated dangerous substances from construction
products using harmonized test methods according to the provisions of the respective technical
committees for European product standards are not available.
The product contains no dangerous substances on the REACH Candidate list or the Norwegian priority
list, and a water-based release agent is used. Based on this it is assumed that the product has a
negligible impact on the indoor environment.
Soil and water
The EPD does not give information on release of dangerous substances to soil and water because the
horizontal standards on measurement of release of regulated dangerous substances from construction
products using harmonised test methods according to the provisions of the respective technical
committees for European product standards are not available.
Carbon footprint
Carbon footprint has not been worked out for the product.
Page | 14 AS BMGS – Structural stairs and landings
8. References
Bozdağ, Ö., Seçer, M., 2007 – Energy consumption of demolition process is on the average
CML-IA, 2013: Characterisation factors developed by Institute of Environmental Sciences (CML):
University Leiden (NL) – http://www.cml.leiden.edu/software/data-cmlia.html
European Commission Joint Research Centre Institute for Prospective Technological Studies (JCR
2014): End-of-waste criteria for waste plastic for conversion, Seville, 2014, doi:10.2791/13033
Ecoinvent Database (2019): Version 3.6
European Federation of Concrete Admixtures Associations a.i.s.b.l. (EFCA) (2021) EPD-EFC-20210198-
IBG1-EN Environmental Product Declaration Concrete admixtures – Plasticizers and Superplasticizers
Liebherr’s Rental – https://www.liebherr-rental.co.uk/; accessed 7th of June 2023
NIBE, 2022: R<THiNK Online-EPD-Tool
Norwegian EPD foundation, Oslo, 2021: NPCR Part A Construction products and services, Version 2.0
Norwegian EPD foundation, Oslo, 2018: NPCR 020 Part B for Concrete and concrete elements, Version
2.0 (references to EN 15804+A2)
Kiwa-Ecobility Experts, Berlin, 2022: PCR A – General Program Category Rules for Construction
Products from the EPD programme of Kiwa-Ecobility Experts; Version 2.1
REACH Regulation (EC) No 1907/2006 of the European Parliament and of the Council on the
Registration, Evaluation, Authorisation and Restriction of Chemicals (REACH)
https://echa.europa.eu/candidate-list-table, accessed 7th of June 2023
Stichting Bouwkwaliteit (SBK 2019): Assessment Method - Environmental Performance Construction
and Civil Engineering Works (GWW), Rijswijk, Version "3.0 January 2019" incl. amendments July 2019,
Jan 2020
Stichting National Environmental Database (NMD), Rijswijk 2022: Environmental Performance
Assessment Method for Construction Works, Version 1.1.
Stichting National Environmental Database (NMD), Rijswijk, 2019: verification protocol –inclusion data
in the Dutch environmental database
SCHWENK Latvija, SIA (2022) NEPD-3757-2696-EN Environmental Product Declaration CEM II A-M (S-
LL) 52.5 N
United Nations, New York, 2015 - Central Product Classification (CPC) Version 2.1
Standards and laws
EN 15804:2012+A2:2019, Sustainability of construction works – Environmental product declarations -
Core rules for ,the product category of construction products
EN 16757:2022, Sustainability of construction works – Environmental product declarations -Product
Category Rules for concrete and concrete elements
ISO 14025:2006, Environmental labels and declarations – Type III environmental declarations –
Principles and procedures
ISO 14040:2006, Environmental management – Life cycle assessment – Principles and framework
ISO 14044:2006, Environmental management – Life cycle assessment – Requirements and guidelines
ISO 21930:2007, Sustainability in building construction – Environmental declaration of building
products
Page | 15 AS BMGS – Structural stairs and landings
Publisher Mail DE.Ecobility.Experts@kiwa.com
Kiwa - Ecobility Experts Web https://www.kiwa.com/de/de/u
Kiwa GmbH ber-kiwa/ecobility-experts/
Voltastr.5, 13355 Berlin
Germany
Programme operator Mail DE.Ecobility.Experts@kiwa.com
Kiwa - Ecobility Experts Web https://www.kiwa.com/de/de/u
Kiwa GmbH ber-kiwa/ecobility-experts/
Voltastr.5, 13355 Berlin
Germany
Author of the Life Cycle Tel. +371 67 607 900
Assessment Mail latvia@kiwa.com
Inspecta Latvia AS Web https://www.kiwa.com/lv
Skanstes iela 54a
LV-1013 Riga
Latvia
Owner of the declaration Tel. +371 67 272 717
BMGS AS Mail info@bmgs.lv
Tvaika iela 27 Web https://www.bmgs.lv
LV-1005 Riga
Latvia
Kiwa-Ecobility Experts -
established member of
Page | 16 AS BMGS – Structural stairs and landings
