ENVIRONMENTAL-PRODUCT DECLARATION
as per ISO 14025 and EN 15804+A2
Owner of the Declaration Industrieverband Klebstoffe e.V
Publisher Institut Bauen und Umwelt e.V. (IBU)
Programme holder Institut Bauen und Umwelt e.V. (IBU)
Declaration number EPD-FEI-20220021-IBG2-EN
Issue date 01.06.2022
Valid to 31.05.2027
Products based on polyurethane or silane-modified polymer,
group 1
FEICA/EFCC/IVK/DBC
www.ibu-epd.com | https://epd-online.com
1. General Information
FEICA/EFCC/IVK/DBC Products based on polyurethane or silane-
modified polymer, group 1
Programme holder Owner of the declaration
IBU – Institut Bauen und Umwelt e.V. Industrieverband Klebstoffe e.V
Hegelplatz 1 Völklinger Straße 4
10117 Berlin 40219 Düsseldorf
Germany Germany
Declaration number Declared product / declared unit
EPD-FEI-20220021-IBG2-EN 1 kg product based on polyurethane or silane-modified polymer; density
0.85 - 1.8 g/cm³
This declaration is based on the product category rules: Scope:
Reaction resin products, 01.08.2021 This
(PCR checked and approved by the SVR) verified EPD entitles the holder to bear the symbol of the Institut
Bauen und Umwelt e.V. It exclusively applies for products produced in
Europe
Issue date and for a period of five years from the date of issue. This EPD may be
used by
01.06.2022
members of DBC, EFCC, FEICA and IVK and their members provided it
has been
proven that the respective product can be represented by this EPD. For
Valid to
this
31.05.2027 purpose a guideline is available at the secretariats of the four associations.
The members of the associations are listed on the respective websites.
The owner of the declaration shall be liable for the underlying information
and evidence; the IBU shall not be liable with respect to manufacturer
information, life cycle assessment data and evidences.
The EPD was created according to the specifications of EN 15804+A2. In
the following, the standard will be simplified as EN 15804 bezeichnet.
Verification
The standard EN 15804 serves as the core PCR
Independent verification of the declaration and data according to ISO
Dipl.-Ing Hans Peters
14025:2011
(chairman of Institut Bauen und Umwelt e.V.)
internally X externally
Florian Pronold Matthias Schulz,
(Managing Director Institut Bauen und Umwelt e.V.) (Independent verifier)
1 Environmental-Product Declaration - FEICA/EFCC/IVK/DBC - Products based on polyurethane or silane-modified polymer, group 1
2. Product
(requirements 2.3)
2.1 Product description/Product definition
This EPD comprises reactive
products based on polyurethane (PU) or silane-modified
polymer (SMP) with a volatile organic copound (VOC) content
≤1 % (VOC definition according to Decopaint Directive) and a Module 3: Liquid-applied roof waterproofing kits
castor
oil/-derivatives content ≤ 10%. The one- or two-component Reactive products for waterproofing roof constructions which
reactive PU products are applied on
are manufactured using polyols and isocyanates. Reactive site
products based on SMP
polymers are usually manufactured as a one-component
system from polyols and
alkoxysilane in a preliminary stage. The aqueous systems
consist of (a) dispersion and are crosslinked by a dispersible Module 4: Reactive products for liquid-applied bridge deck
isocyanate. The products fulfil waterproofing kits
manifold, often specific, functions in the construction, furnishing
and repair Products for liquid-applied waterproofing for use on concrete
of buildings. The product displaying the highest environmental bridge decks
impacts was used
as a representative product for calculating the Life Cycle
Assessment results
(worst-case approach). For the placing on the market in the
European Module 5: Screed material, floor screeds and decorative
Union/European Free Trade Association (EU/EFTA) with the floors
exception of
Switzerland) products falling under Regulation (EU) No Products for screed/synthetic resin screed for use in floor
305/2011 (CPR) need a constructions
Declaration of Performance taking into consideration either the
relevant
harmonised European standard or the European Technical
Assessment and the CE
marking. For the application and use of the products the Module 6: Reactive products as an adhesive for tiles
respective national
provisions apply. Tile adhesives for internal and external tile installations on
walls, floors
2.2 Application
and ceilings
Products based on polyurethane or silane-modified
polymer, group 1, are used for the following applications:
Module 7: Adhesives and sealants
Module 1: Adhesives for parquet and floor coverings Reactive products for use as:
Parquet adhesives in accordance with EN ISO 17178 for · Structural and repair adhesives
wooden and parquet
floors and flooring adhesives in accordance with EN ISO · Surface and joint sealants
22636 for floor
coverings Applications in accordance with the manufacturer's technical
documentation/declaration of performance
Module 2: Reactive products for protecting and repairing
concrete structures
Module 8: Reactive products for watertight covering kits
Products for increasing the durability of concrete and reinforced
concrete Products for waterproofing floors and/or walls in wet rooms
structures as well as for new concrete and for maintenance and inside buildings
repair work
(requirements 2.1), products for structural
bonding of strengthening materials to an existing concrete
structure
(requirements 2.2) and products for concrete
injection for filling cracks, voids and interstices in concrete Module 9: Reactive products for liquid-applied
2 Environmental-Product Declaration - FEICA/EFCC/IVK/DBC - Products based on polyurethane or silane-modified polymer, group 1
waterproofing
Liquid applied products for waterproofing of buildings
12.2 Door Installation & Fixation:
Fixing interior doors with an OCF
Module 10: Reactive products for waterproofing and/or for
pre-treating mineral substrates
Applications in accordance with the manufacturer's technical 12.3 General Gap Filling:
documentation
Filling of regularly and irregularly shaped spaces
between at least two surfaces made of typical building materials
with a one-component
foam (OCF)
Module Module 13: Sealants for glazing
11: Liquid-applied waterproofing membranes for use Two-component reactive sealants are to be used as the second
beneath ceramic tiling barrier of the
structural hermetic seal in insulating glass units.
Module 14: Bonded glazing sealants
Module 12: One-component
foam (OCF)
One component foam in a can is a one-component, One- and
two-component reactive sealants are used for the bonding of
insulating glass units in the window frame.
self-expanding, ready to use polyurethane foam used 2.3 Technical Data
The density
of the products is between 0,85 and 1,8 g/cm³, other relevant
technical data can
for various construction applications. It consists of be found in the manufacturer’s technical documentation.
a Module 1: Reactive
products as adhesive for parquet and floor coverings
The minimum requirements of EN ISO 17178 and EN ISO
22636 must be maintained.
low viscous semi-fluid in a can that leaves the can as
a Module 2: Reactive
products for protecting and repairing concrete structures
2.1 The requirements on essential characteristics for all
intended uses in
froth and immediately forms a polyurethane foam. accordance with EN 1504-2, Tables 1 and 5 must be
maintained. These are:
- Permeability to CO (EN 1062-6)
2
- Water vapour permeability (EN ISO 7783-1/-2)
12.1 Window & External Door Sealing & - Capillary absorption and permeability to water (EN
Insulation: 1062-3)
- Adhesive strength by pull-off test (EN 1542)
2.2 Essential characteristics for all intended uses in accordance
with EN
Installing mechanically fixed external windows and 1504-4, Tables 3.1 and 3.2 (manufacturer's declaration of
performance)
2.3 Requirements on essential characteristics for all intended
uses in
doors with an OCF, as part of a system including accordance with EN 1504-5, Table 3:
- Injectability (EN 1771)
- Viscosity (EN ISO 3219)
Further essential
sealants and tapes characteristics in accordance with the manufacturer's technical
3 Environmental-Product Declaration - FEICA/EFCC/IVK/DBC - Products based on polyurethane or silane-modified polymer, group 1
documentation/declaration of performance authority test
certificates for liquid-applied products for waterproofing of
Module 3: Liquid-applied buildings
roof waterproofing kits (PG-FLK) must be maintained. The characteristics for the proof
The minimum requirements of EAD 030350-00-0402 Liquid- of usability
applied roof waterproofing kits are to be specified in accordance with the test principles for
must be maintained. The essential characteristics are to be granting general
specified in building authority test certificates for liquid applied polymer
accordance with the European Technical Assessment (ETA, products for
specification no.). waterproofing buildings
Module 4: Reactive Module 10: Reactive
products for liquid-applied bridge deck waterproofing kits products for waterproofing and/or for pre-treating mineral
The minimum requirements of ETAG 033 Liquid-applied bridge substrates
deck waterproofing Name Value Unit
kits must be maintained. The essential characteristics are to be Density acc. to EN ISO 2811-1 700 - 1800 kg/m3
specified in accordance with the European Technical
Shore hardness A acc. to ISO 48-4 >15
Assessment (ETA,
specification no.). Shore hardness D acc. to ISO 48-4 >5
Viscosity acc. to ISO 3219-2 <100 Pas
Module 5: Screed
Other performance characteristics in accordance with
material, floor screeds and decorative floors
the manufacturer's technical documentation/declaration of
The requirements on essential characteristics
performance
according to EN 13813 'Screed material and floor screeds –
Screed
Module
materials – Properties and requirements'/ must be maintained.
11: Liquid-applied waterproofing membranes for use
For synthetic
beneath ceramic tilingThe minimum
resin screeds, these are:
requirements on essential characteristics according to EN
- Bond strength (EN 13892-8)
14891 - Liquid
- Reaction to fire (EN 13501-1)
applied water-impermeable products for use beneath ceramic
Further essential characteristics in accordance with
tiling -
the manufacturer's technical documentation/declaration of
Definitions, specifications and test methods- must be
performance
maintained. These are:
- Initial tensile adhesion strength
Module 6: Reactive
- Tensile adhesion strength after water contact
products as an adhesive for tiles
- Tensile adhesion strength after heat ageing
The requirements on essential characteristics according
- Tensile adhesion strength after freeze-thaw cycles
to EN12004, must be maintained. These are:
- Waterproofing
-Tensile adhesion strength after dry storage (EN
- Crack bridging ability
12004-2)
-Tensile adhesion strength after water immersion (EN
12004-2)
-Tensile adhesion strength after heat ageing (EN
Module 12:
12004-2)
One-Component Foams
-Tensile adhesion strength after freeze/thaw cycles
Physical data
(EN 12004-2)
of the one-component foam must be indicated in accordance
-Open time: Tensile strength (EN 12004-2)
with the respective
Further essential characteristics in accordance with
product standards; these can include, for example:
the manufacturer's technical documentation
Module 7: Adhesives
and sealants
12.1 Window
Performance characteristics in accordance with the
& External Door Sealing & Insulation
manufacturer's technical documentation / declaration of
Tensile
performance
Strength EN 17333-4, Movement Capability EN 17333-4,
Curing
Module 8: Reactive
Pressure EN 17333-2, Thermal conductivity EN 17333-5,
products for watertight covering kits
Sound
The minimum requirements of EAD 030352-00-0503 Liquid
Insulation EN ISO 717-1, Post expansion EN 17333-2
applied watertight covering kits for wet room floors and/or walls
must
be maintained. The essential characteristics are to be specified
in accordance
12.2 Door
with the European Technical Assessment (ETA, specification
Installation & Fixation
no.).
Shear Strength EN 17333-4, Tensile Strength
Module 9: Reactive
EN 17333-4, Compression Strength EN
products for liquid-applied waterproofings
17333-4, Curing pressure EN 17333-2
The minimum requirements of
the test principles regarding the issuing of general building
4 Environmental-Product Declaration - FEICA/EFCC/IVK/DBC - Products based on polyurethane or silane-modified polymer, group 1
• Voluntary data: source, date, title (not part of CE-
marking)
12.3 General [Alternative 3: Product for which no legal provisions for
Gap Filling harmonisation of the EU exist]:
Sagging EN
17333-3 Other performance characteristics in accordance with Performance data of the product with respect to its
the characteristics in accordance with the relevant technical
manufacturer's technical documents/declaration of provision (no CE-marking).
performance.
2.4 Delivery status
Liquid or pasty in containers made of tinplate or
Module 13: plastic packed in separate or combi-containers for the required
Sealants for glazing mixing ratio.
Reactive Packages containing one kg of product in different types of
sealants must comply with EN 1279-4 containers.
Performance Sealants in plastic cartridges and foil packs. Typical container
characteristics in accordance with the manufacturer's technical sizes contain
documentation/declaration of performance 10 to 25 kg of material. For major works, vats containing
approx. 200 kg or
IBCs (intermediate bulk containers) containing 1 tonne or more
are also
Module 14: used. The LCA is based on tinplate, plastic and wood
Bonded glazing sealants packaging.
Reactive
2.5 Base materials/Ancillary materials
sealants must comply with RAL-GZ 716 part 2 and ift-Guideline
Products based on polyurethane or silane-modified
VE-08/4.
polymer with a VOC content ≤1 % and a castor oil/-derivatives
Performance
content ≤10 % usually comprise a reactive polymer and a
characteristics in accordance with the manufacturer's technical
crosslinking system.
documentation/declaration of performance
The polymer component contains polyether and/or polyester
polyols. Crosslinking
Please select one of the following options and delete the
takes place after installation on site. In the case of two-
header of the selected [alternative]:
component systems, this involves the use of pre-polymers and
[Alternative 1a: Product according to the CPR, based on a polymers based on typically Methylene diphenyl diisocyanate
hEN]: (MDI), Toluene
diisocyanate (TDI), Hexamethylene diisocyanate (HDI) or
• Performance data of the product in accordance with the Isophorone diisocyanate (IPDI). The resin mixing ratio is
declaration of performance with respect to its essential adjusted according to the
characteristics according to EN xyz:date, title. stoichiometric requirements. Crosslinking starts directly after
• Voluntary data: source, date, title (not part of CE- the components
marking). have been mixed. There are also one-component reactive
[Alternative 1b: Product according to the CPR, based on an polymer formulations
ETA]: based on PU or SMP which crosslink in the presence of
moisture. They comprise
• Performance data of the product in accordance with the prepolymers based on e.g. MDI, TDI, HDI, IPDI or those with
declaration of performance with respect to its essential alkoxy-silane
characteristics according to ETA no. xyz, date, title. groups in the case of SMP formulations. In formulations with
• Voluntary data: source, date, title (not part of CE- aqueous
marking). dispersions, dispersible isocyanates are used for crosslinking.
[Alternative 2a: Product not harmonised in accordance The formulations
with the CPR but in accordance with other provisions for can contain auxiliary materials such as accelerators, catalysts,
harmonisation of the EU]: wetting
agents, foam regulators and viscosity regulators for fine-tuning
Performance data of the product according to the harmonised the product
standards, based on provisions for harmonization. features. Typically, the products covered by this EPD contain
the
Voluntary data: source, date, title (not part of CE-marking). following ranges of base materials and auxiliaries:
Polyol component: up to approx.
[Alternative 2b: Product harmonized as well in accordance 50 %
with the CPR as with other legal provisions of the EU]: Crosslinking component: up to
approx. 95 %
• Performance data of the product in accordance with the SMP component: up to approx. 80 %
declaration of performance with respect to its essential Plasticiser: ~ 0-25 %
characteristics according to EN xyz: date, title or ETA Additives / Pigments: ~ 0-30 %
no. xyz, date, title respectively. Water: ~ 0-60 %
• Performance data of the product, based on the VOC: ≤1 % according to the Decopaint Directive (mandatory)
harmonised standards, in accordance with the other Castor oil and derivatives: ≤10 % (mandatory)
provisions for harmonization.
5 Environmental-Product Declaration - FEICA/EFCC/IVK/DBC - Products based on polyurethane or silane-modified polymer, group 1
These ranges are average values and the composition of 2.6 Manufacture
products complying with the EPD can deviate from these The components of the formulation are usually mixed
concentration levels in individual batch-wise and packaged for delivery.
cases. More detailed information is available in the respective
2.7 Environment and health during manufacturing
manufacturer's
documentation (e.g. product data sheets). As a general rule, no other environmental
Note: For companies to declare their products within protection measures other than those specified by law are
the scope of this EPD it is not sufficient to simply comply with necessary.
the product composition
2.8 Product processing/Installation
shown above. The application of this EPD is only possible for
Products based on polyurethane or silane-modified
member companies
polymer, are processed by trowelling/knife-coating or rolling,
of DBC, EFCC, FEICA, and IVK member associations and only
pouring,
for specific
spraying or injection.
formulations with a total score below the declared maximum
score for a product
group according to the associated guidance document.
Precautions for safe handling and storage (e.g. air
exchange, exhaust ventilation, personal protective measures,
1. substances from the “Candidate
precautions required
List of Substances of Very High Concern for
in the handling of isocyanates, conditions for safe storage)
Authorisation” (SVHC)
must be observed
If this
in accordance with the information on the safety data sheet.
product contains substances listed in the candidate list (latest
version) 2.9 Packaging
exceeding 0.1 percentage by mass, the relevant information
A detailed description of packaging is provided
can be found in the
in section 2.4. Empty containers and clean foils can be
safety data sheet of the relevant product covered by this model
recycled.
EPD.
2. CMR substances in categories 1A 2.10 Condition of use
and 1B During the use phase, products based on
If polyurethane or silane-modified polymer are crosslinked and
this product contains other carcinogenic, mutagenic, reprotoxic essentially
(CMR) comprise an inert three-dimensional network. They are long-
substances in categories 1A or 1B which are not on the lasting products
candidate list, which protect our buildings in the form of adhesives, coatings or
exceeding 0.1 percentage by mass, the relevant information sealants as
can be found in the well as make an essential contribution in retaining their function
safety data sheet of the relevant product covered by this model and long-term
EPD. value.
3. Biocide products added to the
construction product 2.11 Environment and health during use
If Option 1: Products for applications outside indoor
this construction product contains biocide products, the active areas with permanent stays by people
substances,
information on the concentration and/or concentration range,
the product type
together with information on their hazardous properties are During use, the reactive products lose their reactive
listed in the properties and become inert. No risks are known for water, air
safety data sheet of the respective product. and soil if the
products are used as designated.
6 Environmental-Product Declaration - FEICA/EFCC/IVK/DBC - Products based on polyurethane or silane-modified polymer, group 1
water. They are
often used to protect building structures from harmful water
ingress or the effects of flooding.
Option 2: Products for applications inside
indoor areas with permanent stays by people Mechanical destruction
Mechanical destruction of cured reactive products
based on polyurethane or silane-modified polymer does not
lead to any
When used in indoor areas with permanent stays by decomposition products which are harmful to the environment
people, evidence of the emission performance of construction or health.
products in
contact with indoor air must be submitted according to national 2.14 Re-use phase
requirements According to present knowledge, no environmentally
(see chapter 7). No further influences by emissions on the harmful effects are generally anticipated in landfilling, for
environment and example, as a
health are known. result of de-construction and recycling of building materials with
adherent
2.12 Reference service life crosslinked products. If the crosslinked products can be
Cured products based on polyurethane or removed from
silane-modified polymer fulfil manifold, often specific functions construction products without large effort, thermal recovery is a
in the construction practical
or refurbishment of building structures. They decisively improve recycling variant on account of their energy content. Minor
the usability adhesion is not
of building structures and significantly extend their original taken into consideration during disposal. It does not interfere
service lives. with the disposal/recycling of the remaining
The anticipated reference service life depends on the specific components/building materials.
installation
situation and the exposure associated with the product. It can 2.15 Disposal
be influenced by Residual material which cannot be used or recycled
weathering as well as mechanical or chemical loads. must be combined at a specified ratio and hardened. Hardened
Description of the influences on the ageing of the product when product residue is
applied in accordance with the rules of technology. not special waste. Non-hardened product residue is hazardous
waste. Empty, dried
containers (free of drops and scraped clean) are directed to the
2.13 Extraordinary effects recycling
Fire process. Residue must be directed to proper waste disposal
Even without any special taking into
fire safety features, cured products based on polyurethane or consideration the local guidelines. The following waste codes
silane-modified polymer comply according to the
with at least the requirements of EN 13501-1 standard for fire European List of Waste (2000/532/EC) can apply:
classes E and Hardened product residue:
Efl. In terms of the volumes applied, they have only a marginal European Waste Calalogue (EWC) code 080112 (waste paint
influence on and varnish with the exception of
the fire performance characteristics (e.g. smoke gas that mentioned in 08 01 11)
development) of the EWC code 080410 (waste adhesives and sealants other than
building structure in which they have been installed. As mentioned in 08 04 09)
crosslinked
polyurethane systems do not melt or drip, they do not 2.16 Further information
contribute towards More information is available on the
spreading fire. manufacturer's product or safety data sheets and on the
Water manufacturer's websites or on request. Valuable technical
Cured reactive products based on polyurethane or information is also
silane-modified polymer are chemically inert and insoluble in available on the associations' websites.
3. LCA: Calculation rules
environmental impact (worst-case scenario).
3.1 Declared Unit
This EPD refers to the declared unit of 1 kg of
product based on polyurethane or silane-modified polymer,
group 1; applied Depending on the application, a corresponding
into the building with a density of 0.85 - 1.8 g/cm³ in conversion factor such as the density to convert volumetric use
accordance with the IBU to mass must be
PCR part B for reaction resin products. taken into consideration.
The results of the Life Cycle Assessment provided in
this declaration have been selected from the product with the
highest
7 Environmental-Product Declaration - FEICA/EFCC/IVK/DBC - Products based on polyurethane or silane-modified polymer, group 1
The Declaration type is according to EN 15804: Cradle to gate The building deconstruction (demolition process) takes
with options, modules C1–C3, and place in the C1 module which considers energy production and
module D (A1–A3, C, D) and additional modules. consumption in terms
of diesel and all the emissions connected with the fuel-burning
Declared unit
process to run
Name Value Unit
the machines. After the demolition, the product is transported to
Declared unit 1 kg the
Gross density 0.85 - 1.8 g/cm³ end-of-life processing (C2 module) where all the impacts
Conversion factor to 1 kg - - related to the
transport processes are considered. For precautionary principle
For IBU core EPDs (where clause 3.6 is part of the EPD): for
and as a worst-case scenario, thermal treatment is the only
average EPDs, an estimate of the robustness of the LCA
end-of-life scenario considered. This
values must be made, e.g. concerning variability of the
is modelled by the incineration process (module C3) where the
production process, geographical representativeness and the
product ends its life
influence of background data and preliminary products
cycle.
compared to the environmental impacts caused by actual
production.
Module D accounts for potential benefits that are
beyond the defined system boundaries. Credits are generated
3.2 System boundary
during the
Modules A1, A2 and A3 are taken into consideration in
incineration of wastes and related electricity produced that are
the LCA:
occurring in the A5
module.
3.3 Estimates and assumptions
- A1 Production of preliminary products
For this EPD formulation and production data defined
and collected by FEICA were considered. Production waste
was assumed
to be disposed of by incineration without credits as a worst-
- A2 Transport to the plant
case.
- A3 Production incl. provision of energy,
An average of steel and plastic containers, and wooden
production of packaging as well as auxiliaries and consumables
pallets was considered in the LCA.
and waste
treatment 3.4 Cut-off criteria
All raw materials submitted for the formulations and
production data were taken into consideration.
- A4 Transport to site
The manufacture of machinery, plant and other
infrastructure required for the production of the products under
- A5 Installation, product applied into the building review was not
during A5 phase operations and packaging disposal. This stage taken into consideration in the LCA.
considers VOC
emissions during the installation phase. The declared product
does not contain substances
in the formulation that directly emit (as) VOC, but VOCs are Transport of packaging materials is excluded.
generated by a chemical reaction that are occurring during this
phase. The end of life for the 3.5 Background data
packaging material considered is described below: Data from the GaBi database SP40 (2020) was
used as background data.
3.6 Data quality
-Incineration, for materials like Representative products were applied for this EPD and
plastic and wood. the product in the group displaying the highest environmental
impact was
selected for calculating the LCA results. The background data
sets used are less
-Landfill, for inert material like than 4 years old.
metals (where used).
Production data and packaging are based on details
-C1-C2-C3-D provided by the manufacturer. The formulation used for
evaluation refers to a
specific product.
8 Environmental-Product Declaration - FEICA/EFCC/IVK/DBC - Products based on polyurethane or silane-modified polymer, group 1
3.9 Allocation
Mass allocation has been applied when primary data
The data quality of the background data is considered have been used and implemented into the LCA model.
to be good.
3.10 Comparability
3.7 Period under review Basically, a comparison or an evaluation of EPD data is only
Representative formulations are valid for 2021. possible if all the data sets to be compared were created
according to EN 15804 and the building context, respectively
3.8 Geographic Representativeness the product-specific characteristics of performance, are taken
Land or region, in which the declared product system is into account.
manufactured, used or handled at the end of the product´s The used background database has to be mentioned.
lifespan: Europe
4. LCA: Scenarios and additional technical information
Characteristic product properties
Assembly (A5)
Information on biogenic carbon
Name Value Unit
The packaging material contains biogenic carbon Other resources for packaging material 0.1 kg
content which is presented below. Material loss 0.01 kg
Information on describing the biogenic Carbon Content at Material
factory gate loss regards the amount of product not used during the
Name ValueUnit application phase
into the building. This amount is 1% of the product,
kg
Biogenic carbon content in product - impacts related to the production of this part are charged to the
C
A5 module.
Biogenic carbon content in accompanying kg
0.016 This percentage is considered as waste to disposal and
packaging C
impacts of its end of
life have been considered in the LCA model and declared in A5.
The following technical scenario information is required for the
declared modules and optional for non-declared modules.
Modules for which no information is declared can be deleted; In case a reference service life according to applicable ISO
additional information can also be listed if necessary. standards is declared then the assumptions and in-use
conditions underlying the determined RSL shall be declared. In
The following technical information is a basis for the declared addition, it shall be stated that the RSL applies for the reference
modules or can be used for developing specific scenarios in the conditions only.
context of a building assessment if modules are not declared
(MND). The same holds for a service life declared by the manufacturer.
Corresponding information related to in-use conditions needs
A5 is not declared including the disposal of the packaging not be provided if a service life taken from the list on service life
material on the construction site, the amounts of packaging by BNB is declared.
materials included in the LCA calculations must be declared as
technical scenario information for Module A5.
End of life (C1-C3)
Name Value Unit
Collected as mixed construction waste 1 kg
Transport to the building site (A4)
Incineration 1 kg
Name Value Unit
Transport distance 1000 km
Gross weight 34 - 40 t
Payload capacity 27 t
9 Environmental-Product Declaration - FEICA/EFCC/IVK/DBC - Products based on polyurethane or silane-modified polymer, group 1
5. LCA: Results
In Table 1 "Description of the system boundary", all declared modules shall be indicated with an "X"; all modules that are not declared
shall be indicated with "MND" (As default the modules B3, B4, B5 are marked as MNR – module not relevant). In the following tables,
columns can be deleted for modules that are not declared. Indicator values should be declared with three valid digits (eventually using
exponential form (e.g. 1,23E-5 = 0,0000123). A uniform format should be used for all values of one indicator.
If several modules are not declared and therefore have been deleted from the table, the abbreviations for the indicators can be
replaced by the complete names, while the readability and clear arrangement should be maintained; the legends can then be deleted.
If due to relevant data gaps, an indicator cannot be declared in a robust way, then the abbreviation “IND” (indicator not declared)
should be used for this indicator.
• 0 - calculated value is 0
• 0 - value falls under the cut-off
• 0 - assumption which exclude any flows (e.g. exported
electricity A1-A3)
• IND – in cases where the inventory does not support
the methodological approach or the calculation of the
specific indicator IND shall be used.
If no reference service life is declared (see chapter 2.13 "Reference Service Life"), the LCA results of the modules B1-B2 and B6-B7
shall refer to a period of one year. This shall then be indicated as an explanatory text below the tables. In addition, the formula for the
quantification of such B-modules over the total life cycle shall be provided.
DESCRIPTION OF THE SYSTEM BOUNDARY (X = INCLUDED IN LCA; ND = MODULE OR INDICATOR NOT DECLARED; MNR =
MODULE NOT RELEVANT)
BENEFITS
AND LOADS
CONSTRUCTION
BEYOND
PRODUCT STAGE PROCESS USE STAGE END OF LIFE STAGE
THE SYSTEM
STAGE
BOUNDARIE
S
la ire ta m w a Ry lp p u s tro p s n a rT g n iru tc a fu n a M e h t m o rf tro p s n a rTe tis e h t o t e ta g y lb m e s s A e s U e c n a n e tn ia M ria p e R tn e m e c a lp e R tn e m h s ib ru fe R y g re n e la n o ita re p Oe s u re ta w la n o ita re p Oe s u n o itc u rts n o c -e Dn o itilo m e d tro p s n a rT g n is s e c o rp e ts a W la s o p s iD -e s u e R-y re v o c e R-g n ilc y c e Rla itn e to p
A1 A2 A3 A4 A5 B1 B2 B3 B4 B5 B6 B7 C1 C2 C3 C4 D
X X X X X MND MND MNR MNR MNR MND MND X X X MND X
RESULTS OF THE LCA - ENVIRONMENTAL IMPACT according to EN 15804+A2: 1 kg of product based on polyurethane or
silane modified polymer, group 1
Parameter Unit A1-A3 A4 A5 C1 C2 C3 D
GWP-total kg CO 2 eq 4.79E+00 5.27E-02 1.8E-01 2.79E-04 1.24E-02 2.21E+00 -9.5E-01
GWP-fossil kg CO 2 eq 4.81E+00 5.22E-02 9.38E-02 2.66E-04 1.18E-02 2.21E+00 -9.47E-01
GWP-biogenic kg CO 2 eq -3.57E-02 1.52E-04 8.62E-02 1.24E-05 5.42E-04 8.82E-05 -2.23E-03
GWP-luluc kg CO 2 eq 4.5E-03 4.22E-04 4.84E-05 6.39E-09 2.79E-07 2.08E-05 -6.66E-04
ODP kg CFC11 eq 6.76E-09 6.27E-18 6.76E-11 2.84E-20 1.24E-18 2.62E-16 -9.93E-15
AP mol H+ eq 1.02E-02 1.56E-04 1.29E-04 3.6E-06 3.73E-05 1.31E-03 -1.33E-03
EP-freshwater kg P eq 1.93E-05 1.59E-07 1.98E-07 5.75E-11 2.51E-09 4.4E-08 -1.23E-06
EP-marine kg N eq 2.67E-03 6.96E-05 3.5E-05 1.63E-06 1.72E-05 6.31E-04 -3.43E-04
EP-terrestrial mol N eq 2.93E-02 7.8E-04 4.11E-04 1.79E-05 1.89E-04 7.26E-03 -3.68E-03
kg NMVOC
POCP 9.47E-03 1.38E-04 7.2E-03 4.91E-06 3.39E-05 1.62E-03 -9.87E-04
eq
ADPE kg Sb eq 8.18E-06 3.74E-09 8.22E-08 8.06E-12 3.52E-10 4.65E-09 -1.56E-07
ADPF MJ 1.05E+02 6.94E-01 1.11E+00 3.81E-03 1.66E-01 5.87E-01 -1.61E+01
m3 world eq
WDP 1.34E+00 4.66E-04 2.69E-02 5.27E-07 2.3E-05 2.17E-01 -9.86E-02
deprived
GWP = Global warming potential; ODP = Depletion potential of the stratospheric ozone layer; AP = Acidification potential of land and water; EP =
Eutrophication potential; POCP = Formation potential of tropospheric ozone photochemical oxidants; ADPE = Abiotic depletion potential for non-fossil
resources; ADPF = Abiotic depletion potential for fossil resources; WDP = Water (user) deprivation potential)
RESULTS OF THE LCA - INDICATORS TO DESCRIBE RESOURCE USE according to EN 15804+A2: 1 kg of product based on
polyurethane or silane modified polymer, group 1
Parameter Unit A1-A3 A4 A5 C1 C2 C3 D
PERE MJ 6.67E+00 3.9E-02 6.65E-01 1.2E-05 5.25E-04 8.23E-02 -3.52E+00
PERM MJ 5.85E-01 0 -5.85E-01 0 0 0 0
PERT MJ 7.26E+00 3.9E-02 7.99E-02 1.2E-05 5.25E-04 8.23E-02 -3.52E+00
PENRE MJ 8.33E+01 6.95E-01 1.63E+00 3.81E-03 1.67E-01 2.21E+01 -1.61E+01
10 Environmental-Product Declaration - FEICA/EFCC/IVK/DBC - Products based on polyurethane or silane-modified polymer, group 1
PENRM MJ 2.2E+01 0 -5.2E-01 0 0 -2.15E+01 0
PENRT MJ 1.05E+02 6.95E-01 1.11E+00 3.81E-03 1.67E-01 5.87E-01 -1.61E+01
SM kg 0 0 0 0 0 0 0
RSF MJ 0 0 0 0 0 0 0
NRSF MJ 0 0 0 0 0 0 0
FW m3 4.03E-02 4.52E-05 7.22E-04 2.16E-08 9.41E-07 5.11E-03 -4.08E-03
PERE = Use of renewable primary energy excluding renewable primary energy resources used as raw materials; PERM = Use of renewable primary
energy resources used as raw materials; PERT = Total use of renewable primary energy resources; PENRE = Use of non-renewable primary energy
excluding non-renewable primary energy resources used as raw materials; PENRM = Use of non-renewable primary energy resources used as raw
materials; PENRT = Total use of non-renewable primary energy resources; SM = Use of secondary material; RSF = Use of renewable secondary fuels;
NRSF = Use of non-renewable secondary fuels; FW = Use of net fresh water
RESULTS OF THE LCA – WASTE CATEGORIES AND OUTPUT FLOWS according to EN 15804+A2:
1 kg of product based on polyurethane or silane modified polymer, group 1
Parameter Unit A1-A3 A4 A5 C1 C2 C3 D
HWD kg 1.12E-05 3.23E-08 1.12E-07 3.7E-13 1.62E-11 3.34E-10 -6.41E-09
NHWD kg 1.66E-01 1.06E-04 4.75E-02 3.9E-07 1.7E-05 1.11E-02 -7.44E-03
RWD kg 2.34E-03 8.6E-07 2.54E-05 4.09E-09 1.79E-07 2.37E-05 -1.2E-03
CRU kg 0 0 0 0 0 0 0
MFR kg 0 0 0 0 0 0 0
MER kg 0 0 0 0 0 0 0
EEE MJ 0 0 2.12E-01 0 0 0 0
EET MJ 0 0 3.86E-01 0 0 0 0
HWD = Hazardous waste disposed; NHWD = Non-hazardous waste disposed; RWD = Radioactive waste disposed; CRU = Components for re-use;
MFR = Materials for recycling; MER = Materials for energy recovery; EEE = Exported electrical energy; EET = Exported thermal energy
RESULTS OF THE LCA – additional impact categories according to EN 15804+A2-optional:
1 kg of product based on polyurethane or silane modified polymer, group 1
Parameter Unit A1-A3 A4 A5 C1 C2 C3 D
Disease
PM ND ND ND ND ND ND ND
incidence
IR kBq U235 eq ND ND ND ND ND ND ND
ETP-fw CTUe ND ND ND ND ND ND ND
HTP-c CTUh ND ND ND ND ND ND ND
HTP-nc CTUh ND ND ND ND ND ND ND
SQP SQP ND ND ND ND ND ND ND
PM = Potential incidence of disease due to PM emissions; IR = Potential Human exposure efficiency relative to U235; ETP-fw = Potential comparative
Toxic Unit for ecosystems; HTP-c = Potential comparative Toxic Unit for humans (cancerogenic); HTP-nc = Potential comparative Toxic Unit for humans
(not cancerogenic); SQP = Potential soil quality index
Potential Human exposure efficiency relative to U235,
Disclaimer 1 – This impact category deals mainly with the eventual impact of
low dose ionizing radiation on human health of the nuclear fuel cycle. It does
not consider effects due to possible nuclear accidents, occupational exposure or radioactive waste disposal in underground facilities.
Potential ionizing
radiation from the soil, radon and (from) some construction materials is
also not measured by this indicator.
ADP minerals & metals, ADP fossil, WDP, ETF-fw,
HTP-c, HTP-nc, SQP, Disclaimer 2 – The results of this environmental impact
indicator shall be used with care as the uncertainties on these results are
high or as there is limited experience with the indicator.
Additional
environmental impact indicators (suggested by EN15804, table 4) are not
declared in the EPD. The results of this environmental impact indicator shall
be used with care as the uncertainties on these results are high and as there
is limited experience with the indicator (see ILCD classification in EN 15804,
table 5). For this reason, results based on these indicators are not considered
suitable for a decision-making process and are thus not declared in the EPD.
11 Environmental-Product Declaration - FEICA/EFCC/IVK/DBC - Products based on polyurethane or silane-modified polymer, group 1
6. LCA: Interpretation
The majority of impacts are associated with the production required for the generation and supply of electricity. It should be
phase (A1-A3). The most significant noted that
contribution to the production phase impacts is the upstream Primary Energy Demand – Renewable (PERT) generally
production of raw represents a small
materials as the main driver. Another substantial contributor in percentage of the production phase primary energy demand
the production with the bulk of the
phase, in the category of Abiotic depletion potential demand coming from non-renewable energy resources.
for nonfossil
resources (ADPminerals&
metals), is the
steel sheet used as a packaging material. Emissions Transportation
associated with the to the construction site (A4) and the installation process (A5)
manufacturing of products also have some influence on the make a low
Formation potential of tropospheric contribution to all impacts.
ozone (POCP) in the production phase. In all EPDs, CO
2
is the most important contributor to Global Warming Potential
(GWP). For the
Acidification Potential (AP), NOx and SO contribute the largest The
2
installation phase influences mainly the Photochemical ozone
share. In some cases, HCl in water also impacts AP due to the
formation indicator,
use
due to the emission of VOC during the operations. These
of TiO as a pigment.
2 emissions are not directly
related to the pre-products in the resins, but they are related to
the
reaction products between pre-products and air components
The
(water and oxygen).
majority of life cycle energy consumption takes place during the
production
phase (A1-A3). Significant contributions to Primary Energy
Demand –
The
Non-renewable (PENRT) come from the energy resources used
end-of-life phases influence climate change indicators, due to
in the production of
the incineration
raw materials. The largest contributor to Primary Energy
processes occurring in the C3 module, the process used for
Demand – Renewable
modelling the thermal treatment process of the resin.
(PERT) impacts comes from the consumption of renewable
energy resources
7. Requisite evidence
VOC
- or documentation
of test data that are required in
Special tests and evidence have not been carried out
or provided within the framework of drawing up this Model EPD.
Some member
states require special documentation on VOC emissions into any of the existing regulations or in any of the existing
indoor air for voluntary labelling programs for low-emitting products, as far as
specific areas of application. This documentation, as well as these
documentation for
voluntary VOC labelling, has to be provided separately and is
specific for
product in question. (1) include limits for the parameters
TVOC, TSVOC, carcinogens, formaldehyde, acetaldehyde, LCI
limits for individual
substances (including but not limited to the European list of
harmonized LCIs),
and the R value;
Evidence pertaining to VOC emissions shall show
(2) base their test methods on EN 16516;
- either an
attestation of compliance with, (3) perform testing and apply the limits
after 28 days of storage in a ventilated test chamber, under the
12 Environmental-Product Declaration - FEICA/EFCC/IVK/DBC - Products based on polyurethane or silane-modified polymer, group 1
conditions
specified in EN 16516; some regulations and programs also
have limits after 3
days, on top of the 28 days limits; - Each carcinogen:
1 µg/m³
(4) express the test results as air
concentrations in the European Reference Room, as specified - Formaldehyde:
in EN 16516. 100 µg/m³
- LCI: different
per substance involved
Examples of such regulations are the Belgian Royal
Decree C-2014/24239, or the German AgBB/ ABG. Examples - R value: 1
of such voluntary (meaning that, in total, 100 % of the combined LCI values must
labelling programs are EMICODE, Blue Angel or Indoor Air not be exceeded).
Comfort. Informative Annexes (2 tables):
Table 1 shown below is an overview of the most
relevant regulations and specifications as of October 2021, as
regards
requirements after 3 days of storage in a ventilated test
chamber.
Table 2 provides an overview of the most
relevant regulations and specifications as of October 2021, as
Relevant test results shall be produced either by an ISO regards
17025 accredited commercial test lab or by a qualified internal requirements after 28 days of storage in a ventilated test
test lab of chamber. Some details
the manufacturer. Examples for the applied limits after 28 days may be missing in the table due to lack of space. Values given
of storage in a represent
ventilated test chamber are: maximum values/limits.
- TVOC: 1000 µg/m³
- TSVOC: 100 µg/m³
13 Environmental-Product Declaration - FEICA/EFCC/IVK/DBC - Products based on polyurethane or silane-modified polymer, group 1
7.1 VOC emissions the regulating authorities must pass the test to AgBB achieving
The following information on the product's emission at least the result of "suitable for use in interior applications".
performance in accordance with the AgBB diagram: For products availing of an EMICODE EC 1 PLUS classification
- Test institute or an emission test to RAL-UZ 113 (Blue Angel for Installation
- Measurement process Materials), the requirements concerning emission performance
- Date of test report to AgBB are automatically applied as satisfied. The
- AgBB overview of results corresponding measured values are to be indicated. If this is
- Result/Interpretation not possible the permissible limit values are to be indicated.
Products applied in interior applications which are regulated by
8. References
ETAG 033 hardness- Part 4:
Liquid applied Indentation hardness by durometer method (Shore hardness)
bridge deck waterproofing kits
EN ISO 717-1
ISO 48-4 EN ISO
ISO 48-4:2018, 717-1:2020 Acoustics - Rating of sound insulation in buildings
Rubber, vulcanized or thermoplastic - Determination of and of
14 Environmental-Product Declaration - FEICA/EFCC/IVK/DBC - Products based on polyurethane or silane-modified polymer, group 1
building elements - Part 1: Airborne sound insulation 3219:1994-10, Plastics - Polymers/resins in the liquid state or
as
EN 1062-3 emulsions or dispersions - Determination of viscosity using a
EN rotational
1062-3:2008-04, Paints and varnishes - Coating materials and viscometer with defined shear rate
coating
systems for exterior masonry and concrete - Part 3: ISO 3219-2
Determination of liquid ISO
water permeability 3219-2:2021, Rheology - Part 2: General principles of rotational
and
EN 1062-6 oscillatory rheometry
EN
1062-6:2002-10, Paints and varnishes - Coating materials and EN ISO 7783
coating EN ISO
systems for exterior masonry and concrete - Part 6: 7783:2019-02, Paints and varnishes - Determination of water-
Determination of carbon vapour
dioxide permeability transmission properties - Cup method
EN 1279-4 EN 12004
EN 1279-4:2002 EN12004:2012,
Glass in building - Insulating glass units - Part 4: Methods of Adhesives for ceramic tiles
test for the
physical attributes of edge seals EN 12004-1
EN 12004-1:2017, Adhesives
EN 1504-2 for ceramic tiles – Part 1: Requirements, assessment and
EN verification of
1504-2:2004-12, Products and systems for the protection and constancy of performance, classification and marking
repair of
concrete structures - Definitions, requirements, quality control EN 12004-2
and evaluation EN
of conformity - Part 2: Surface protection systems for concrete 12004-2:2017, Adhesives for ceramic tiles - Part 2: Test
methods
EN 1504-4
EN EN 13501-1
1504-4:2004-11, Products and systems for the protection and EN
repair of concrete 13501-1:2018, Fire classification of construction products and
structures - Definitions, requirements, quality control and building
evaluation of elements - Part 1: Classification using data from reaction to fire
conformity- Part 4: Structural bonding tests
EN 1504-5 EN 13813
EN EN
1504-5:2004-12, Products and systems for the protection and 13813:2002-10, Screed material and floor screeds - Screed
repair of materials -
concrete structures - Definitions, requirements, quality control Properties and requirements
and evaluation
of conformity - Part 5: Concrete injection EN 13892-8
EN
EN 1542 13892:2003-02, Methods of test for screed materials - Part 8:
EN Determination
1542:1999-07, Products and systems for the protection and of bond strength
repair of
concrete structures - Test methods - Measurement of bond ISO 14025
strength by pull-off
DIN EN ISO
EN 1771 14025:2011-10, Environmental labels and declarations — Type
EN III environmental
1771:2004-11, Products and systems for the protection and declarations — Principles and procedures
repair of
concrete structures - Test methods - Determination of EN 14891
injectability and EN
splitting test 14891:2012-04, Liquid applied water impermeable products for
use beneath
ISO 2811-1 ceramic tiling - Definitions, specifications and test methods
ISO
2811-1:2016, Paints and varnishes - Determination of density - EN 15804
Part 1: Pycnometer method
EN
EN ISO 3219 15804:2019+A2, Sustainability of construction works —
EN ISO Environmental Product Declarations
15 Environmental-Product Declaration - FEICA/EFCC/IVK/DBC - Products based on polyurethane or silane-modified polymer, group 1
— Core rules for the product category of construction products
Belgian Royal
EN 16516 Decree C-2014/24239
EN 16516:2017
Belgisch Staatsblad 8 MEI 2014, p. 60603. — Koninklijk besluit
Construction products - Assessment of release of dangerous tot vaststelling
substances - van de drempelniveaus voor de emissies naar het binnenmilieu
Determination of emissions into indoor air van bouwproducten
voor bepaalde geoogde gebruiken
EN ISO 17025
EN ISO 17025:2018-03 Blue Angel
Environmental
General requirements for the competence of testing and label organised by the federal
calibration laboratories government of
Germany www.blauer-engel.de
EN ISO 17178
EN ISO CPR
17178:2020-06, Adhesives - Adhesives for bonding parquet to CPR Regulation
subfloor - (EU) No 305/2011 of the European Parliament and of the
Test methods and minimum requirements Council of 9 March 2011
laying down harmonised conditions for the marketing of
EN 17333-2 construction products
EN and repealing Council Directive 89/106/EEC
17333-2:2020+AC:2020, Characterisation of one component
foam - Decopaint
Part 2: Expansion characteristics Directive
Directive
EN 17333-3 2004/42/CE of the European Parliament and the council of 21
EN April 2004 on the
17333-3:2020, Characterisation of one component foam - Part limitation of emissions of volatile organic compounds due to the
3: Application use of organic
solvents in certain paints and varnishes and vehicle refinishing
EN 17333-4 products and
EN amending Directive 1999/13/EC
17333-4:2020, Characterisation of one component foam - Part
4: Mechanical EMICODE
strength
EMICODE, GEV – Gemeinschaft Emissionskontrollierte
EN 17333-5 Verlegewerkstoffe, Klebstoffe und Bauprodukte e. V.
EN (pub.).www.emicode.de
17333-5:2020, Characterisation of one component foam - Part
5: Insulation GaBi 10
software & documentation
EN ISO 22636 Data base for
EN ISO Life Cycle Engineering LBP, University of Stuttgart and Sphera,
22636:2020, Adhesives - Adhesives for floor coverings - documentation
Requirements for of GaBi 10 data sets http://documentation.gabi-software.com/,
mechanical and electrical performance 2020
EAD German AgBB
030350-00-0402
EAD Committee for
030350-00-0402:2018-08, Liquid Applied Roof Waterproofing Health-related Evaluation of Building Products: health-related
Kits evaluation of
emissions of volatile organic compounds (VOC and SVOC)
EAD from building products;
030352-00-0503 status: June 2012
EAD 030352-00-0503:2019-01, Liquid
applied watertight covering kits for wet room floors and/or walls www.umweltbundesamt.de/produkte/bauprodukte/agbb.htm
2000/532/EC IBU 2021
Commission Institut Bauen und Umwelt e.V.: General
decision dated 3 May 2000 replacing decision 94/3/EC on a Instructions for the EPD programme of Institut Bauen und
waste directory in Umwelt e.V. EPD
accordance with Article 1 a) of Council Directive 75/442/EEC on programme. Version 2.0. Berlin: Institut Bauen und Umwelt
waste and e.V., 2021
Council decision 94/904/EC on a directory of hazardous waste
in terms of www.ibu-epd.com
Article 1, paragraph 4 of Directive 91/689/EEC on hazardous
waste ift-Guideline VE-08/4
16 Environmental-Product Declaration - FEICA/EFCC/IVK/DBC - Products based on polyurethane or silane-modified polymer, group 1
ift-Guideline VE-08/4:2017,
Beurteilungsgrundlage für geklebte Verglasungssysteme
Indoor Air
Comfort
Product
certification by Eurofins, Hamburg, Germany
www.eurofins.com
PCR Part A
Product
Category Rules for Building-Related Products and Services,
Part A: Calculation
Rules for the Life Cycle Assessment and Requirements on the
Project report,
Version 1.1, Institut Bauen und Umwelt e.V., 2021-01
PCR Part B
Product
Category Rules for Construction Products, Part B: Reaction
resin products, Institut
Bauen und Umwelt e.V., 2019-01
RAL-GZ 716
RAL-GZ 716:2019-04 part 2,
Kunststoff-Fensterprofilsysteme - Gütesicherung
REACH
17 Environmental-Product Declaration - FEICA/EFCC/IVK/DBC - Products based on polyurethane or silane-modified polymer, group 1
18 Environmental-Product Declaration - FEICA/EFCC/IVK/DBC - Products based on polyurethane or silane-modified polymer, group 1
Directive (EG)
No. 1907/2006 of the European Parliament and of the Council
dated 18 December
2006 on the registration, evaluation, approval and restriction of
chemical
substances (REACH), for establishing a European Agency for
chemical substances,
for amending Directive 1999/45/EC and for annulment of
Directive (EEC) No.
793/93 of the Council, Directive (EC) No. 1488/94 of the
Commission, Guideline
76/769/EEC of the Council and Guidelines 91/155/EEC,
93/67/EEC, 93/105/EC and
2000/21/EC of the Commission.
The literature referred to in the Environmental Product
Declaration must be listed in full.Standards already fully quoted
in the EPD do not need to be listed here again.
The current version of PCR Part A and PCR Part B of the PCR
document on which they are based must be referenced.
19 Environmental-Product Declaration - FEICA/EFCC/IVK/DBC - Products based on polyurethane or silane-modified polymer, group 1
Publisher
Institut Bauen und Umwelt e.V. +49 (0)30 3087748- 0
Hegelplatz 1 info@ibu-epd.com
10117 Berlin www.ibu-epd.com
Germany
Programme holder
Institut Bauen und Umwelt e.V. +49 (0)30 3087748- 0
Hegelplatz 1 info@ibu-epd.com
10117 Berlin www.ibu-epd.com
Germany
Author of the Life Cycle Assessment
Sphera Solutions GmbH +49 711 341817-0
Hauptstraße 111- 113 info@sphera.com
70771 Leinfelden-Echterdingen www.sphera.com
Germany
Owner of the Declaration
Industrieverband Klebstoffe e.V +49 (0)211 67931-10
Völklinger Straße 4 info@klebstoffe.com
40219 Düsseldorf www.klebstoffe.com
Germany
Deutsche Bauchemie e.V. +49 (0)69 2556-1318
Mainzer Landstr. 55 info@deutsche-bauchemie.de
60329 Frankfurt www.deutsche-bauchemie.de
Germany
FEICA - Association of the European Adhesive and +32 (0)267 673 20
Sealant Industry info@feica.eu
Avenue E. van Nieuwenhuyse 2 www.feica.eu
B-1160 Brussels
Belgium
EFCC - European Federation for Construction +32289720-39
Chemicals info@efcc.be
Boulevard du Triomphe 172 www.efcc.eu
1160 Brussels
Belgium
20 Environmental-Product Declaration - FEICA/EFCC/IVK/DBC - Products based on polyurethane or silane-modified polymer, group 1
