—
EPD
Environmental Product Declaration
PT1 VG4-S
Production site: ABB AG Ratingen
DOCUMENT KIND IN COMPLIANCE WITH
Environmental Product Declaration ISO 14025 and EN50693
PROGRAM OPERATOR PUBLISHER
The Norwegian EPD Foundation The Norwegian EPD Foundation
REGISTRATION NUMBER OF THE PROGRAM OPERATOR ISSUE DATE
11.11.2022
NEPD-3888-2843-EN
VALID TO STATUS SECURITY LEVEL
11.11.2027 Approved Public
OWNING ORGANIZATION DECLARATION NUMBER REV. LANG. PAGE
ABB Switzerland Ltd 3XAA008725 A001 en 1/18
© Copyright 2022 ABB. All rights reserved.
ENVIRONMENTAL PRODUCT DECLARATION
EPD Owner ABB Swizerland Ltd, Group Technology Management
Manufacturer name and ABBAG
address Oberhausener Str. 33, 40472 Ratingen
Organization no CHE-101.538.426
Seila Rodriguez-Vilches–seila.rodriguez-vilches@ch.abb.com
Company contact
Sustainability Product Manager
The Norwegian EPD Foundation
Post Box 5250 Majorstuen, 0303 Oslo, Norway
Program operator
Ph.:+47 23 08 80 00
email: post@epd-norge.no
PT1 VG4-S
FU: The functional unit of this study is a single pole part
which provides high dielectric strength as well as better
protection of the vacuum interrupter against environmental
Declared product &
influences, humidity, and mechanical forces during a
Functional unit or declared unit
reference service life of 20 years.
RF: The reference flow is a single PT1 pole part including
related accessories and packaging.
PT1 pole parts are used for the vacuum circuitbreakers
which are used in electrical distribution for control and
protection of cables, overhead lines, transformer and
distribution substations, motors, transformers, generators
Product description
and capacitor banks. The scope of the Medium voltage
circuit breakers is to interrupt an electric current which flows
via vacuum interrupters which is embedded in the pole part
with a mechanical actuator.
46211 - Electrical apparatus for switching or protecting
CPC code electrical circuits, or for making connexions to or in electrical
circuits, for a voltage exceeding 1000 V
Independentverification of the declaration and data carried
out according to ISO 14025: 2010.
☐ INTERNAL ☒ EXTERNAL
Third party verification carried out by: EPD Norway:
Independent verification Anne Rønning
Signature:
Håkon Hauan, CEO EPD-Norge
Approved by
Signature:
Core PCR: EPDItaly007 – PCR for Electronic and Electrical
Reference PCR and version Products and Systems, Rev. 2, 2020/01/20.
number Sub PCR: EPDItaly012 - Electronic and electrical products and
systems – Switches, Rev. 0, 2020/03/16.
EN -50693:2019 - Product category rules for life cycle
Core PCR assessments of electronic and electrical products and
systems
STATUS SECURITY LEVEL DOCUMENT ID. REV. LANG. PAGE
Approved Public 3XAA008725 A001 en 2/18
© Copyright 2022 ABB. All rights reserved.
ENVIRONMENTAL PRODUCT DECLARATION
Product RSL description 20 years
World (raw materials),
Markets of applicability Germany (production, use and end-of-life)
Europe (use and end-of-life)
This EPD is based on the LCA study described in the LCA
LCA study
report 3XAA008724.
EPD type Product specific
EPD scope “Cradle to grave”
Year of reported primary data 2021
2B Srl (Italy)
Technical support
Via della Chiesa Campocroce 4, Mogliano Veneto (TV)
LCA software SimaPro 9.3.0.2 (2021)
LCI database ecoinvent v3.8 (2021)
LCIA methodology EN -50693:2019
EPDs published within the same product category, though
originating from different programs, may not be compa-
Comparability rable. Full conformance with a PCR allows EPD comparability
only when all stages of a life cycle have been considered.
However, variations and deviations are possible.
The owner of the declaration shall be liable for the
underlying information and evidence. EPD Norway shall not
Liability
be liable with respect to manufacturer, life cycle assessment
data and evidences.
STATUS SECURITY LEVEL DOCUMENT ID. REV. LANG. PAGE
Approved Public 3XAA008725 A001 en 3/18
© Copyright 2022 ABB. All rights reserved.
ENVIRONMENTAL PRODUCT DECLARATION
Contents
ABB Purpose & Embedding Sustainability .....................................................................................5
General Information ........................................................................................................................ 6
Constituent materials ...................................................................................................................... 7
LCA background information ......................................................................................................... 8
Inventory analysis .......................................................................................................................... 12
Environmental indicators ..............................................................................................................14
Additional environmental information ........................................................................................ 16
References....................................................................................................................................... 17
STATUS SECURITY LEVEL DOCUMENT ID. REV. LANG. PAGE
Approved Public 3XAA008725 A001 en 4/18
© Copyright 2022 ABB. All rights reserved.
ENVIRONMENTAL PRODUCT DECLARATION
ABB Purpose & Embedding Sustainability
ABB is a leading global technology company that energizes the transformation of society
and industry to achieve a more productive, sustainable future. By connecting software to
its electrification, robotics, automation and motion portfolio, ABB pushes the boundaries
of technology to drive performance to new levels. With a history of excellence stretching
back more than 130 years, ABB’s success is driven by about 110 thousand talented employ-
ees in over 100 countries.
ABB's Electrification business offers a wide-ranging portfolio of products, digital solu-
tions and services, from substation to socket, enabling safe, smart and sustainable elec-
trification. Offerings encompass digital and connected innovations for low and medium
voltage, including EV infrastructure, solar inverters, modular substations, distribution au-
tomation, power protection, wiring accessories, switchgear, enclosures, cabling, sensing
and control.
ABB is committed to continually promoting and embedding sustainability across its op-
erations and value chain, aspiring to become a role model for others to follow. With its
ABB Purpose, ABB is focusing on reducing harmful emissions, preserving natural re-
sources and championing ethical and human behavior.
STATUS SECURITY LEVEL DOCUMENT ID. REV. LANG. PAGE
Approved Public 3XAA008725 A001 en 5/18
© Copyright 2022 ABB. All rights reserved.
ENVIRONMENTAL PRODUCT DECLARATION
General Information
The range of ABB Ratingen includes innovative and smart systems, with components and
services for power distribution and switching and control technology. The product range
of the Ratingen plant includes components such as vacuum interrupters, pole parts, cir-
cuit breakers, current limiters and core modules for the production of primary gas-insu-
lated switchgear. These components are widely used in associated plants within the
worldwide ABB value chain as well as by OEM partners in the industry.
ABB DE-ELDS adopts and implements for its own activities an integrated Quality/Environ-
mental/Health Management System in compliance with the following standards:
ISO 9001/2015 - Quality Management Systems- Requirements
ISO 14001/2015 - Environmental management systems -Requirements
ISO 45001:2018- Occupational health and safety management systems
The product Embedded Pole, Type PT1 VG4-S declared in this LCA includes one main ver-
sion.
Technical information
Product Name PT1 VG4-S
Rated voltage [kV] 12 - 17,5
Rated current [A] ... 1250
Rated short circuit breaking current [kA] ... 31,5
A key component of PT1 pole part is a vacuum interrupter. The main purpose of the vac-
uum interrupter is to interrupt a current flow by separation of the electrical contacts re-
sults in a metal vapor arc, which is quickly extinguished. The vacuum interrupter and its
terminals are completely embedded in thermoplastic material. In such cases, high dielec-
tric strength can be achieved. The pole part provides better protection against environ-
mental influences, humidity and mechanical forces and enables an easy adaptation on the
circuit-breaker drive. The maintenance-free vacuum interrupter and the thermoplastic
pole part housing accumulate in a form-fit unit which is not final product and cannot be
used without a drive. A vacuum circuit breaker consists of the pole parts and a drive, which
has to create and store energy to move contact within vacuum interrupter.
The vacuum circuit breakers are used in electrical distribution for control and protection
of cables, overhead lines, distribution substations, motors, transformers, generators and
capacitor banks. The scope of the medium voltage circuit breakers is to interrupt an elec-
tric current with a mechanical actuator (spring mechanism) or a magnetic actuator.
The manufacturing of the pole parts is located in ABB Ratingen, where the pole parts are
produced on the injection molding machine and in the assembling line. All components
and some of the subassemblies are produced by ABB’s suppliers and are then assembled
in the factory or used in the injection molding machine.
STATUS SECURITY LEVEL DOCUMENT ID. REV. LANG. PAGE
Approved Public 3XAA008725 A001 en 6/18
© Copyright 2022 ABB. All rights reserved.
ENVIRONMENTAL PRODUCT DECLARATION
Constituent materials
The PT1 VG4-S pole part weights about 5,6 kg. One of the components was excluded be-
cause of lack of data, as their mass is estimated to be well below 2% of the total weight,
according to the PCR EPDItaly-012 cut-off criteria.
Materials Name CAS Number Product weight [kg] %
Plastics Polyamide glass filled --- 1,2 21,6
Other plastics and rubbers --- 0,2 3,6
Metals Steel 7439-89-6 0,8 14,5
Copper 7440-50-8 2,5 44,4
Aluminium 7429-90-5 0,5 8,6
Chromium 7440-47-3 0,1 1,4
Silver 7440-22-4 0,01 0,2
Others Ceramics 66402-68-4 0,3 5,5
Others --- 0,01 0,2
Total 5,6 100
Silver; 0,01 kg;
Other; 0,01 kg; 0,2%
0,2%
Ceramics; 0,3 kg; 5,5%
Polyamide GF; 1,2 kg;
Steel; 0,8 kg; 14,5%
Other plastics and
rubbers;
Chromium; 0,1 kg; 1,4% 0,2 kg; 3,6%
Aluminium; 0,5 kg; 8,6%
Copper; 2,5 kg; 44,4%
Diagrammtitel
The single-use packaging and reusable packaging is also included in the analysis,
specifically in the manufacturing core stage. The single-use and reusable packaging for
PT1 are composed of the same materials, mainly of steel fixing brackets, a cardboard box
and a wooden pallet. Additionally, in both packaging versions, further items are in use.
Polyethylene-foam, Puma-Folie® hermetic VAS and a desiccation bag. A reusable box can
be used for 15 circulations, a polyethylene-foam is used for 20 circulations. The rest of the
packaging material is for single use only. ABB receives packaging components from out-
side suppliers and packages the pole parts before shipping them.
STATUS SECURITY LEVEL DOCUMENT ID. REV. LANG. PAGE
Approved Public 3XAA008725 A001 en 7/18
© Copyright 2022 ABB. All rights reserved.
ENVIRONMENTAL PRODUCT DECLARATION
LCA background information
Functional Unit
The functional unit of this study is a single pole part which provides high dielectric
strength as well as better protection of the vacuum interrupter against environmental in-
fluences, humidity, and mechanical forces during a reference service life of 20 years. The
reference flow is a single PT1 pole part including related accessories and packaging.
System Boundaries
For the analysis of the product a life cycle model is applied in form of a “Cradle to Grave”
model. It covers the following main life cycle stages: manufacturing, including the relevant
upstream process (e.g. acquisition of raw material, preparation of semi-finished goods,
etc.) and the main manufacturing and processing steps; distribution; installation, includ-
ing the relevant steps for the preparation of the product for use; use including the re-
quired maintenance steps within the RSL (reference service life of the product) associated
to the reference product; end-of-life stage, including the necessary steps until final dis-
posal or recovery of the product system.
The following table shows the stages of the product life cycle and the information stages
according to EN -50693 for the evaluation of electronic and electrical products and sys-
tems.
The stages of the product life cycle and the information considered for the evaluation of
PT1 VG4-S are:
STATUS SECURITY LEVEL DOCUMENT ID. REV. LANG. PAGE
Approved Public 3XAA008725 A001 en 8/18
© Copyright 2022 ABB. All rights reserved.
ENVIRONMENTAL PRODUCT DECLARATION
 Manufacturing upstream includes raw materials, and production activities of ABB
suppliers, including transport of semifinished items and subassemblies to ABB
Ratingen site.
 The core part of the manufacturing stage includes local consumptions (ABB Rat-
ingen) the relevant assembling and waste due to manufacturing as well as the
packaging production.
 The distribution stage includes the impacts related to the distribution of the prod-
uct at the installation site.
 The installation stage includes the end of life of the packaging.
 The use and maintenance stages include the impact related to energy consump-
tion during the service life of the product.
 The end-of-life stage includes all activities related to waste treatment and dis-
posal of the product at the end of its service life.
Temporal and geographical boundaries
The ABB component suppliers are sourced all over the world. All primary data collected
from ABB are from 2021, which is a representative production year. Secondary data are
also representative for this year, as provided by ecoinvent v3.8.
The selected ecoinvent processes in the LCA model have global representativeness, due to
the unclear origin of each component. In this way, a conservative approach has been
adopted.
The results of this study are only applicable to PT1 VG4-S produced in Ratingen in 2021.
Boundaries in the life cycle
As indicated in the PCR EPDItaly012, capital goods, such as buildings, machinery, tools
and infrastructure, the packaging for internal transport which cannot be allocated directly
to the production of the reference product, may be excluded from the system boundary.
Infrastructures, when present, such as processes deriving from the ecoinvent database
have not been excluded.
Data quality
In this EPD, both primary and secondary data are used. Site specific foreground data have
been provided by ABB. The main data sources are the bill of materials available on the
enterprise resource planning. For all processes for which primary are not available, generic
data originating from the ecoinvent v3.8 database, allocation cut-off by classification, are
used. The ecoinvent database is available in the SimaPro 9.3.0.2 software used for the cal-
culations.
STATUS SECURITY LEVEL DOCUMENT ID. REV. LANG. PAGE
Approved Public 3XAA008725 A001 en 9/18
© Copyright 2022 ABB. All rights reserved.
ENVIRONMENTAL PRODUCT DECLARATION
Environmental impact indicators
The information obtained from the inventory analysis is aggregated according to the ef-
fects related to the various environmental issues. According to PCR EPDItaly007 and EN -
50693 the environmental impact indicators must be determined using the characteriza-
tion factors and impact assessment methods specified in EN 15804:2012+A2:2019.
PCR EPDItaly007 and the EN -50693 standards establish four indicators for climate impact
(GWP-GHG): GWP (total) which includes all greenhouse gases; GWP (fossil fuels); GWP (bi-
ogenic carbon) which includes the emissions and absorption of biogenic carbon dioxide
and biogenic carbon stored in the product; GWP (land use and land use change).
Allocation rules
An allocation key is used for consumptions related to the manufacturing process in the
production site as well for company waste and product distribution. Since the factory pro-
duces several products (components, apparatus and switchgears), only a part of the en-
vironmental impact has been allocated to the specific production line.
The values for the electricity, heat, pressurized air and water consumptions have been read
and recorded from the counters which are distributed in the whole factory and are con-
nected to the certain areas or even single machines or single workstations.
For the end-of-life allocation, the “polluter pays” principle is adopted according to what is
defined in the CEN/TR 16970 standard, as required by the PCR EPDItaly007. This means,
waste treatment processes are allocated to the product system that generates the waste
until the end-of-waste state is reached. The environmental burdens of recycling and en-
ergy recovery processes are therefore allocated to the product system that generates the
waste, while the product system that uses the exported energy and recycled materials
receives it burden-free. However, the potential benefits and avoided loads from recovery
and recycling processes are not considered because it is not required by EPDItaly007.
Limitations and simplifications
The raw material life cycle stage includes the extraction of raw materials but neglects the
production of various components at ABB’s suppliers (e.g. grease), as their mass repre-
sents less than 2% of that of the whole PT1 pole part, as stated in the paragraph of cut-
off criteria of EPDItaly-012: “Materials making up the switch it-self whose total mass does
not exceed 2% of the total weight of the device”.
Due to the fact that a PCR EPDItaly012 has been published for switches and not for com-
ponents of the “switch”, like a pole part or a vacuum interrupter, a PCR EPDItaly007 has
been used as a principal one for this study and a PCR EPDItaly012 was taken into account
as a reference, for example for the calculation of the USE AND MAINTENANCE STAGE or
regulation of cut-off criteria, specifically excluding of the materials whose total mass does
not exceed 2% of the total weight of the device.
This same applies for packaging, where small parts, such as sticking labels, is even a
smaller fraction of the total mass.
STATUS SECURITY LEVEL DOCUMENT ID. REV. LANG. PAGE
Approved Public 3XAA008725 A001 en 10/18
© Copyright 2022 ABB. All rights reserved.
ENVIRONMENTAL PRODUCT DECLARATION
Surface treatments like silver plating, copper plating have been considered in the LCA
model. Primer, oiled treatments have been excluded by operational choice. Phosphating is
not available in selected libraries (ecoinvent and industry data 2.0). Therefore, a zinccoat-
ing process was used instead of phosphating treatment. Both methodologies are used to
protect steel parts against rusting and other types of corrosion.
Scraps for metal working and plastic processes are included when already defined in
ecoinvent.
STATUS SECURITY LEVEL DOCUMENT ID. REV. LANG. PAGE
Approved Public 3XAA008725 A001 en 11/18
© Copyright 2022 ABB. All rights reserved.
ENVIRONMENTAL PRODUCT DECLARATION
Inventory analysis
The ecoinvent v3.8 cut-off by classification system processes are used to model the back-
ground system of the processes. In addition, polyoxymethylene and electrogalvanized
steel were taken from the database Industry Data 2.0, available in SimaPro libraries, as it
is not present in ecoinvent database.
All components in the pole part, raw material inputs are modelled with data from ecoin-
vent representing a global market coverage. These datasets are assumed to be repre-
sentative.
Manufacturing stage
The pole part is composed of several components all of which are made from different
materials. Most of the inputs to the products’ manufacturing stage are already produced
components. Copper is the most frequently used material, followed by Polyamide GF and
steel. All steel components (hot rolled, galvanized, low-alloyed steel, unalloyed) are mod-
elled accordingly.
The single-use packaging and reusable packaging is also included in the analysis in the
manufacturing core stage including all elements and components belonging to
packaging. ABB receives packaging components from outside suppliers and packages the
pole parts before shipping them.
The transport distances from raw materials suppliers to the manufacturing is not known.
However, this information is included in the data sets of ecoinvent “market for”. The dis-
tance from the subassembly or single parts manufacturing factory to ABB facility is calcu-
lated. In the factory, the different components and subassemblies are assembled into the
pole part. All the components are produced by ABB’s suppliers.
The energy mix used for the production phase is representative for Ratingen production
site and includes an autonomous combined heat and power plant (CHP) driven by natural
gas.
The waste generated by the production and assembly processes is included in the calcu-
lation.
Distribution
The transport distances from ABB plant to the place of use were exactly defined. There
are four customers identified. The reference port is Rotterdam, NL.
Installation
The installation phase only implies manual activities and no energy is consumed. This
phase also includes the disposal of the packaging of the PT1 pole part.
STATUS SECURITY LEVEL DOCUMENT ID. REV. LANG. PAGE
Approved Public 3XAA008725 A001 en 12/18
© Copyright 2022 ABB. All rights reserved.
ENVIRONMENTAL PRODUCT DECLARATION
Use
Use and maintenance are modelled according to the PCR EPDItaly012 – Switches for the
PT1.
For the use phase, the general European medium voltage electricity mix from ecoinvent
v3.8 is used.
Since no maintenance happens during the use phase, the environmental impacts linked
this procedure have been omitted from the analysis.
During the use phase, the PT1 dissipates some electricity due to ohmic losses. Electricity
consumption was calculated with the following formula:
P * 8760 * RSL *α
E [kWh]= use
use 1000
P =R*(0.5*I)2
use
α=0.3
with
 P = Power losses
use
 E = Energy losses
use
 RSL = Reference Servise Lifetine
 R = Resistance
 I = Rated Current which is flowing through component during steady-state
 8760 h =The number of hours in a year
 α is a coefficient describing the amount of time in which the switch is re-
quested to operate its function
Parameters Country code
Internal resistance [µΩ] 21
Nominal current [A] 1250
P [W] 6,83
use
E [kWh] 358,89
use
End-of-life
The transport distances from the place of use to the place of disposal are assumed to be
100 km.
The end-of-life stage is modelled according to PCR EPDItaly012 and IEC/TR 62635. The
percentages for end-of-life treatments of pole parts are taken from IEC/TR 62635, while
the data for packaging waste scenarios are provided by EUROSTAT.
STATUS SECURITY LEVEL DOCUMENT ID. REV. LANG. PAGE
Approved Public 3XAA008725 A001 en 13/18
© Copyright 2022 ABB. All rights reserved.
ENVIRONMENTAL PRODUCT DECLARATION
Environmental indicators
The following tables show the environmental impact indicators of the life cycle of a single
pole part of type PT1 VG4-S, as indicated by PCR EPDItaly007, PCR EPDItaly012 and EN -
50693:2019.
The indicators are divided into the contribution of the processes to the different modules
(upstream, core and downstream) and stages (manufacturing, distribution, installation,
use and end-of-life).
UPSTREAM CORE DOWNSTREAM
Impact category Unit Total
Manufacturing Distribution Installation Use End of life
Climate change kg CO2 eq 2,30E+02 7,54E+01 6,13E+00 1,25E+00 3,61E-01 1,46E+02 1,31E+00
Climate change-Fossil kg CO2 eq 2,24E+02 7,45E+01 6,04E+00 1,25E+00 3,91E-02 1,41E+02 1,20E+00
Climate change-Biogenic kg CO2 eq 5,99E+00 8,96E-01 8,32E-02 3,43E-04 3,21E-01 4,58E+00 1,10E-01
Climate change-Land use and LU change kg CO2 eq 4,24E-01 8,81E-02 2,28E-03 7,62E-04 3,63E-05 3,32E-01 9,68E-04
Ozone depletion kg CFC11 eq 1,28E-05 4,85E-06 6,41E-07 2,65E-07 3,56E-09 6,97E-06 8,96E-08
Acidification mol H+ eq 2,83E+00 2,02E+00 2,04E-02 2,94E-02 1,46E-04 7,58E-01 4,25E-03
Eutrophication, freshwater kg P eq 3,02E-01 1,59E-01 2,30E-03 5,32E-05 5,56E-06 1,41E-01 2,44E-04
Photochemical ozone formation kg NMVOC eq 8,44E-01 4,88E-01 1,88E-02 2,17E-02 1,50E-04 3,12E-01 3,53E-03
Depletion of abiotic resources – minerals
and metals kg Sb eq 5,12E-02 4,97E-02 1,21E-03 2,10E-06 1,53E-07 3,30E-04 9,61E-06
Depletion of abiotic resources – fossil fuels MJ 3,98E+03 8,78E+02 7,86E+01 1,72E+01 3,34E-01 2,99E+03 1,22E+01
Water use (AWARE) m3 7,34E+01 3,96E+01 9,94E-01 4,14E-02 8,97E-04 3,25E+01 1,98E-01
UPSTREAM CORE DOWNSTREAM
Resource use parameters Unit Total
Manufacturing Distribution Installation Use End of life
MJ, low
Use of n-renew.prim. energy(ener.) PENRE cal. value 3,93E+03 8,30E+02 7,75E+01 1,72E+01 3,34E-01 2,99E+03 1,22E+01
MJ, low
Use ofrenew. prim. energy (ener.) PERE cal. value 6,38E+02 1,13E+02 7,24E+00 1,54E-01 1,44E-02 5,17E+02 8,34E-01
MJ, low
Use of n-renew.prim. energy(mat.) PENRM cal. value 4,88E+01 4,76E+01 1,16E+00 0,00E+00 0,00E+00 0,00E+00 0,00E+00
MJ, low
Use ofrenew. prim. energy (mat.) PERM cal. value 6,05E+00 0,00E+00 6,05E+00 0,00E+00 0,00E+00 0,00E+00 0,00E+00
Total use of non-renew primar energy res (PENRT) MJ 3,98E+03 8,78E+02 7,86E+01 1,72E+01 3,34E-01 2,99E+03 1,22E+01
Total use ofrenewable primar energy res (PERT) MJ 6,44E+02 1,13E+02 1,33E+01 1,54E-01 1,44E-02 5,17E+02 8,34E-01
Net use of fresh water (from AWARE) m3 3,55E+00 1,02E+00 2,84E-02 1,39E-03 6,87E-05 2,50E+00 6,53E-03
Use of secondary material kg 9,10E-01 9,08E-01 2,62E-03 0,00E+00 0,00E+00 0,00E+00 0,00E+00
Use of renewable secondary fuels MJ 0,00E+00 0,00E+00 0,00E+00 0,00E+00 0,00E+00 0,00E+00 0,00E+00
Use of non-renewable secondary fuels MJ 0,00E+00 0,00E+00 0,00E+00 0,00E+00 0,00E+00 0,00E+00 0,00E+00
PENRE: Use of non-renewable primary energy excluding non-renewable primary energy resources used as raw material; PERE: Use of renewable primary en-
ergy excluding renewable primary energy resources used as raw material; PENRM: Use of non-renewable primary energy resources used as raw material;
PERM: Use of renewable primary energy resources used as raw material; PENRT: Total use of non-renewable primary energy resources (primary energy and
primary energy resources used as raw materials); PERT: Total use of renewable primary energy resources (primary energy and primary energy resources used
as raw materials).
STATUS SECURITY LEVEL DOCUMENT ID. REV. LANG. PAGE
Approved Public 3XAA008725 A001 en 14/18
© Copyright 2022 ABB. All rights reserved.
ENVIRONMENTAL PRODUCT DECLARATION
UPSTREAM CORE DOWNSTREAM
Waste production indicators Unit Total
Manufacturing Distribution Installation Use End of life
Hazardous waste disposed kg 8,50E-03 7,04E-03 3,50E-04 2,56E-05 7,01E-07 1,06E-03 1,97E-05
Non-hazardous waste disposed kg 2,79E+01 1,56E+01 4,08E-01 6,29E-01 4,13E-02 9,92E+00 1,29E+00
Radioactive waste disposed kg 2,42E-02 1,94E-03 1,01E-04 1,18E-04 1,71E-06 2,20E-02 5,08E-05
Materials for energy recovery kg 1,08E+00 1,41E-01 6,99E-01 0,00E+00 2,05E-01 0,00E+00 3,31E-02
Materials for recycling kg 6,89E+00 1,60E+00 7,11E-01 0,00E+00 2,41E-01 0,00E+00 4,33E+00
Exported thermal energy MJ 4,63E+00 6,50E-01 3,12E+00 0,00E+00 7,37E-01 0,00E+00 1,25E-01
Exported electricity energy MJ 2,34E+00 3,29E-01 1,58E+00 0,00E+00 3,68E-01 0,00E+00 6,37E-02
STATUS SECURITY LEVEL DOCUMENT ID. REV. LANG. PAGE
Approved Public 3XAA008725 A001 en 15/18
© Copyright 2022 ABB. All rights reserved.
ENVIRONMENTAL PRODUCT DECLARATION
Additional environmental information
Recyclability potential
The recyclability potential of the reference product is calculated by dividing “MFR: material
for recycling” with the total weight of the pole part. This is based on the end-of-life sce-
nario adopted from IEC/TR 62635 Edition 1.0 which is representative for Europe. The sce-
nario is based on the rates given for materials that go through a separation process, and
the production losses in the recycling processes have also been considered; thus, a con-
servative approach is adopted. Recyclability potentials for other relay configurations are
also provided, which is based on a sensitivity analysis and extrapolation procedures.
Recyclability potential
PT1 VG4-S 85,75 %
Additional Norwegian requirements
Greenhouse gas emissions from the use of electricity in the manufactu-
ring phase
The energy mix used for the production phase is representative for Ratingen production
site and includes an autonomous combined heat and power plant (CHP) driven by natural
gas.
Data source Amount Unit
Ecoinvent 3.8 heat and power co-generation, natural gas 0,6015 kg CO2-eq/kWh
Dangerous substances
The product contains no substances given by the REACH candidate list.
Indoor environment
The product meets the requirements for low emissions.
Carbon footprint
Carbon footprint has not been worked out for the product.
STATUS SECURITY LEVEL DOCUMENT ID. REV. LANG. PAGE
Approved Public 3XAA008725 A001 en 16/18
© Copyright 2022 ABB. All rights reserved.
ENVIRONMENTAL PRODUCT DECLARATION
References
 Deminenko, W. (2022) PT1 VG4-S: Life Cycle Assessment Report, Doc. no
3XAA008724, ABB Switzerland Ltd, Group Technology Management. EN -
50693:2019 - Product category rules for life cycle assessments of electronic and
electrical products and systems
 EN 15804:2012+A2:2019 – Sustainability of constructions – Environmental prod-
ucts declarations (September 2019)
 PCR EPDItaly007 - Electronic and electrical products and systems (rev.2), October
2020
 PCR EPDItaly012 - Electronic and electrical products and systems - Switches,
March 2020
 IEC/TR 62635 - Guidelines for end-of-life information provided by manufacturers
and recyclers and for recyclability rate calculation of electrical and electronic
equipment - Edition 1.0 2012-10
 ISO 14040:2006 - Environmental management -Life cycle assessment - Principles
and framework
 ISO 14044:2006 - Environmental management - Life cycle assessment - Require-
ments and guidelines
 Ecoinvent, 2021. Swiss Centre for Life Cycle Assessment, v3.8 (www.ecoinvent.ch).
 PRé Consultants, 2021. Software SimaPro versione 9.2.0.1 (www.pre.nl).
 https://ec.europa.eu/eurostat
 General Programme Instructions for The Norwegian EPD Foundation/EPD-Norge
(www.epd-norge.no) version 5:2019
 EPDItaly Regulations rev. 5.0 (1st July 2020)
 EN System boundaries +A2:2019 – Sustainability of constructions - Environmental
product declarations (September 2019)
STATUS SECURITY LEVEL DOCUMENT ID. REV. LANG. PAGE
Approved Public 3XAA008725 A001 en 17/18
© Copyright 2022 ABB. All rights reserved.
ENVIRONMENTAL PRODUCT DECLARATION
Program Operator and
Ph. +47 23 08 80 00
publisher
The Norwegian EPD
Foundation
Post Box 5250 Majorstuen,
email: post@epd-norge.no
0303 Oslo
Norway web www.epd-norge.no
Owner of the declaration
ABB Swizerland Ltd, Group
Technology Management
Brown Boveri Straße 6, 5400
web www.abb.com
Baden, Switzerland
Author of the life cycle
Ph. +49 160 9947 3144
assessment
Wadim Deminenko
ABB AG e-mail: wadim.deminenko@de.abb.com
Oberhausener Str. 33, 40472
web www.abb.com
Ratingen, Germany
STATUS SECURITY LEVEL DOCUMENT ID. REV. LANG. PAGE
Approved Public 3XAA008725 A001 en 18/18
© Copyright 2022 ABB. All rights reserved.
