ver1 2015
ENVIRONMENTAL PRODUCT DECLARATION
in accordance with ISO 14025, ISO 21930 and EN 15804
Owner of the declaration: Pipelife Sverige AB
Program operator: The Norwegian EPD Foundation
Publisher: The Norwegian EPD Foundation
Declaration number: NEPD-2999-1674-EN
Registration number: NEPD-2999-1674-EN
ECO Platform reference number: -
Issue date: 12.08.2021
Valid to: 12.08.2026
PVC Sewage pipe 250x7,3 SN8 3m
Pipelife Sverige AB
www.epd-norge.no
NEPD-2999-1674-EN PVC Sewage pipe 250x7,3 SN8 3m
1 / 8
General information
Product: Owner of the declaration:
PVC Sewage pipe 250x7,3 SN8 3m Pipelife Sverige AB
Contact person:
Phone: +46 513 22114
e-mail: yvette.lennartsson@pipelife.com
Program operator: Manufacturer:
Pipelife Sverige AB
The Norwegian EPD Foundation
Pb. 5250 Majorstuen, 0303 Oslo
Phone: +47 23 08 80 00
e-mail: post@epd-norge.no
Declaration number: Place of production:
Pipelife Sverige AB
NEPD-2999-1674-EN Box 50 SE-524 02 Ljung
Sweden
ECO Platform reference number: Management system:
EN ISO 9001:2015 and EN ISO 14001:2015
This declaration is based on Product Category Rules: Organisation no:
SE556087042901
CEN Standard EN 15804:2012+A1:2013 serves as core PCR
NPCR 019:2018 Part B for Piping systems use in sewage and storm water systems
(under gravity)
Statement of liability: Issue date: 12.08.2021
The owner of the declaration shall be liable for the underlying information and
evidence. EPD Norway shall not be liable with respect to manufacturer Valid to: 12.08.2026
information, life cycle assessment data and evidences.
Declared unit: Year of study:
1 m PVC Sewage pipe 250x7,3 SN8 3m 2021
Declared unit with option: Comparability:
EPD of construction products may not be comparable if they not comply with EN
A1,A2,A3,A4,A5,C1,C2,C3,C4,D
15804 and seen in a building context.
Functional unit: Development and verification of EPD:
The unit is with socket included (one socket/3m) The declaration has been developed and verified using EPD tool lca.tools
ver EPD2020.11, developed by LCA.no AS. The EPD tool is integrated into
the company's environmental management system, and has been
approved by EPD-Norway
General information on verification of EPD from EPD tools:
Independent verification of data, other environmental information and Developer of EPD:
the declaration according to ISO 14025:2010, § 8.1.3 and § 8.1.4. Individual
third party verification of each EPD is not required when the EPD tool is i) Yvette Lennartsson
integrated into the company's environmental management system, ii) the
procedures for use of the EPD tool are approved by EPDNorway, and iii) Reviewer of company-specific input data and EPD:
the proccess is reviewed annualy. See Appendix G of EPD-Norway's
General Programme Instructions for further information on EPD tools. Ove Soderberg
Verification of EPD tool: Approved:
Independent third party verification of the EPD tool, background data
Sign
and test-EPD in accordance with EPDNorway's procedures and guidelines
for verification and approval of EPD tools.
Michael M. Jenssen, Asplan Viak AS
(no signature required) Håkon Hauan, CEO EPD-Norge
NEPD-2999-1674-EN PVC Sewage pipe 250x7,3 SN8 3m
2 / 8
Product
Product description: Technical data:
PVC material with density 1400 kg/m3.
Produced according EN 1401-1:2019.
Product specification Stiffness SN8.
Oil resistant sealing ring according EN 681-1.
Conformity mark covered by certificate; Nordic Poly Mark
Market:
Materials kg % Europe, with scenario made for the Swedish market.
Filler 2,13 22,55
Reference service life, product
Chemicals 0,18 1,88
Lifetime on product calculated more than 100 years.
Rubber, synthetic 0,06 0,63
Polyvinylchloride (PVC) 7,08 74,94 Reference service life, construcion
Total: 9,44
Packaging kg
Packaging 0,02
Packaging 0,31
Total including packaging 9,77
LCA: Calculation rules
Declared unit: Allocation:
The allocation is made in accordance with the provisions of EN 15804.
1 m PVC Sewage pipe 250x7,3 SN8 3m
Incoming energy and water and waste production in-house is allocated
Cut-off criteria: equally among all products through mass allocation. Effects of primary
production of recycled materials is allocated to the main product in which
All major raw materials and all the essential energy is included. The
the material was used. The recycling process and transportation of the
production processes for raw materials and energy flows with very small
material is allocated to this analysis.
amounts (less than 1%) are not included. These cut-off criteria do not
apply for hazardous materials and substances.
Data quality:
Specific data for the product composition are provided by the manufacturer. They represent the production of the declared product and were collected for
EPD development in the year of study. Background data is based on registered EPDs according to EN 15804, Ostfold Research databases, ecoinvent and other
LCA databases. The data quality of the raw materials in A1 is presented in the table below.
Materials Source Data quality Year
Producer
Polyvinylchloride (PVC) Producer specific data, S-PVC 2017
specific
Chemicals ecoinvent 3.5 Database 2018
Filler ecoinvent 3.5 Database 2018
Packaging ecoinvent 3.5 Database 2018
Rubber, synthetic ecoinvent 3.5 Database 2018
NEPD-2999-1674-EN PVC Sewage pipe 250x7,3 SN8 3m
3 / 8
System boundary:
Additional technical information:
Nordic Poly Mark
NEPD-2999-1674-EN PVC Sewage pipe 250x7,3 SN8 3m
4 / 8
LCA: Scenarios and additional technical information
The following information describe the scenarios in the different modules of the EPD.
We assume that the pipes will remain in the ground, therefore no data input to "End of life stage - C" and "Beyond the system bondaries - D".
Transport from production place to user (A4)
Capacity utilisation Fuel/Energy
Type Type of vehicle Distance km Unit Value (l/t)
(incl. return) % consumption
Truck with trailer, EURO 6, 55% degree of
Truck 55,0 % 100 0,022606 l/tkm 2,26
filling by weight
Railway l/tkm
Boat l/tkm
Other Transportation l/tkm
Assembly (A5)
. Unit Value
Auxiliary kg
Water consumption m3
Electricity consumption kWh
Other energy carriers MJ 147,7557
Material loss kg
Output materials from waste treatment kg
Dust in the air kg
VOC emissions kg
¨
NEPD-2999-1674-EN PVC Sewage pipe 250x7,3 SN8 3m
5 / 8
LCA: Results
The LCA results are presented below for the declared unit defined on page 2 of the EPD document.
System boundaries (X=included, MND=module not declared, MNR=module not relevant)
Construction Beyond the
Product stage installation User stage End of life stage . system
stage bondaries
A1 A2 A3 A4 A5 B1 B2 B3 B4 B5 B6 B7 C1 C2 C3 C4 . D
X X X X X MND MND MND MND MND MND MND X X X X . X
Environmental impact
Parameter Unit A1-A3 A4 A5 C1 C2 C3 C4 D
GWP kg CO 2 -eq 1,15E+01 7,78E-02 1,98E+01 0 0 0 0 0
ODP kg CFC11 -eq 1,75E-05 1,60E-08 3,61E-06 0 0 0 0 0
POCP kg C 2H 4-eq 1,71E-03 1,22E-05 3,71E-03 0 0 0 0 0
AP kg SO 2 -eq 3,92E-02 2,01E-04 1,20E-01 0 0 0 0 0
EP kg PO 3- -eq 6,70E-03 2,77E-05 2,69E-02 0 0 0 0 0
4
ADPM kg Sb -eq 1,50E-04 1,85E-07 2,74E-05 0 0 0 0 0
ADPE MJ 3,03E+02 1,28E+00 2,88E+02 0 0 0 0 0
GWP Global warming potential; ODP Depletion potential of the stratospheric ozone layer; POCP Formation potential of tropospheric photochemical oxidants;
AP Acidification potential of land and water; EP Eutrophication potential; ADPM Abiotic depletion potential for non fossil resources; ADPE Abiotic depletion
potential for fossil resources
"Reading example: 9,0 E-03 = 9,0*10-3 = 0,009"
*INA Indicator Not Assessed
waR slairetam tropsnarT gnirutcafunaM tropsnarT ylbmessA esU ecnanetniaM riapeR tnemecalpeR tnemhsibrufeR lanoitarepO ygrene esu lanoitarepO esu
retaw
-eD noitcurtsnoc noitilomed tropsnarT etsaW gnissecorp lasopsiD -yrevoceR-esueR -gnilcyceR laitnetop
NEPD-2999-1674-EN PVC Sewage pipe 250x7,3 SN8 3m
6 / 8
Resource use
Parameter Unit A1-A3 A4 A5 C1 C2 C3 C4 D
RPEE MJ 6,66E+01 2,32E-02 4,05E+00 0 0 0 0 0
RPEM MJ 4,40E+00 0,00E+00 0,00E+00 0 0 0 0 0
TPE MJ 7,10E+01 2,32E-02 4,05E+00 0 0 0 0 0
NRPE MJ 2,19E+02 1,32E+00 2,96E+02 0 0 0 0 0
NRPM MJ 1,48E+02 0,00E+00 0,00E+00 0 0 0 0 0
TRPE MJ 3,67E+02 1,32E+00 2,96E+02 0 0 0 0 0
SM kg 0,00E+00 0,00E+00 2,81E+03 0 0 0 0 0
RSF MJ 1,38E-02 0,00E+00 0,00E+00 0 0 0 0 0
NRSF MJ 0,00E+00 0,00E+00 0,00E+00 0 0 0 0 0
W m3 4,55E+00 3,12E-04 3,72E-01 0 0 0 0 0
RPEE Renewable primary energy resources used as energy carrier; RPEM Renewable primary energy resources used as raw materials; TPE Total use of renewable
primary energy resources; NRPE Non renewable primary energy resources used as energy carrier; NRPM Non renewable primary energy resources used as
materials; TRPE Total use of non renewable primary energy resources; SM Use of secondary materials; RSF Use of renewable secondary fuels; NRSF Use of non
renewable secondary fuels; W Use of net fresh water
"Reading example: 9,0 E-03 = 9,0*10-3 = 0,009"
*INA Indicator Not Assessed
End of life - Waste
Parameter Unit A1-A3 A4 A5 C1 C2 C3 C4 D
HW kg 1,30E-02 7,03E-07 1,51E-04 0 0 0 0 0
NHW kg 2,09E+00 1,20E-01 5,77E+00 0 0 0 0 0
RW kg INA* INA* INA* 0 0 0 0 0
HW Hazardous waste disposed; NHW Non hazardous waste disposed; RW Radioactive waste disposed
"Reading example: 9,0 E-03 = 9,0*10-3 = 0,009"
*INA Indicator Not Assessed
End of life - Output flow
Parameter Unit A1-A3 A4 A5 C1 C2 C3 C4 D
CR kg 0,00E+00 0,00E+00 0,00E+00 0 0 0 0 0
MR kg 3,76E-01 0,00E+00 0,00E+00 0 0 0 0 0
MER kg 2,77E-04 0,00E+00 0,00E+00 0 0 0 0 0
EEE MJ INA* INA* INA* 0 0 0 0 0
ETE MJ INA* INA* INA* 0 0 0 0 0
CR Components for reuse; MR Materials for recycling; MER Materials for energy recovery; EEE Exported electric energy; ETE Exported thermal energy
"Reading example: 9,0 E-03 = 9,0*10-3 = 0,009"
*INA Indicator Not Assessed
NEPD-2999-1674-EN PVC Sewage pipe 250x7,3 SN8 3m
7 / 8
Additional requirements
Greenhouse gas emissions from the use of electricity in the manufacturing phase
National production mix from import, low voltage (production of transmission lines, in addition to direct emissions and losses in grid) of applied electricity for
the manufacturing process (A3).
Electricity mix Data source Amount Unit
El-mix, Sweden (kWh) ecoinvent 3.4 Alloc Rec 42,67 g CO2-ekv/kWh
Dangerous substances
The product contains no substances given by the REACH Candidate list or the national priority list.
Indoor environment
Bibliography
ISO 14025:2010 Environmental labels and declarations - Type III environmental declarations - Principles and procedures.
ISO 14044:2006 Environmental management - Life cycle assessment - Requirements and guidelines.
EN 15804:2012+A1:2013 Environmental product declaration - Core rules for the product category of construction products.
ISO 21930:2017 Core rules for environmental product declarations of construction products.
ecoinvent v3, Allocation, cut-off by classification, Swiss Centre of Life Cycle Inventories.
Iversen et al., (2018) eEPD v3.0 - Background information for EPD generator system. LCA.no report 04.18.
Vold, et al., (2019) EPD generator for Pipelife - Background information for customer application and LCA data. report number 08.19
NPCR Part A: Construction products and services. Ver. 1.0. April 2017, EPD-Norge.
NPCR 019 Part B for Piping systems for use in sewage and storm water systems (under gravity), Ver 2.0.
Program operator and publisher Phone: +47 23 08 80 00
The Norwegian EPD Foundation e-mail: post@epd-norge.no
Post Box 5250 Majorstuen, 0303 Oslo,Norway web: www.epd-norge.no
Owner of the declaration Phone: +46 513 22114
Pipelife Sverige AB e-mail: yvette.lennartsson@pipelife.com
Box 50 SE-524 02 Ljung web:
Author of the Life Cycle Assessment Phone: +47 916 50 916
LCA.no AS e-mail: post@lca.no
Dokka 1C 1671 Kråkerøy web: www.lca.no
Developer of EPD generator Phone: +47 916 50 916
LCA.no AS e-mail: post@lca.no
Dokka 1C,1671 Kråkerøy web: www.lca.no
NEPD-2999-1674-EN PVC Sewage pipe 250x7,3 SN8 3m
8 / 8
