ENVIRONMENTAL PRODUCT DECLARATION
as per ISO 14025 and EN 15804+A2
Owner of the Declaration Ravago Building Solutions
Programme holder Institut Bauen und Umwelt e.V. (IBU)
Publisher Institut Bauen und Umwelt e.V. (IBU)
Declaration number EPD-RAV-20220157-CBD1-EN
Issue date 04.01.2023
Valid to 03.01.2028
RAVATHERMTM XPS (X) PLUS / ULTRA
RAVAGO BUILDING SOLUTIONS
www.ibu-epd.com | https://epd-online.com
Umwelt Produktdeklaration Name des Herstellers – Name des Produkts
General Information
RAVAGO BUILDING SOLUTIONS RAVATHERMTM XPS (X)
PLUS/ULTRA
Programme holder Owner of the declaration
IBU – Institut Bauen und Umwelt e.V. Ravago Building Solutions Germany GmbH
Hegelplatz 1 Value Park Y51
10117 Berlin 06258 Schkopau
Germany Germany
Declaration number Declared product / declared unit
EPD-RAV-20220157-CBD1-EN RAVATHERMTM XPS (X) PLUS and ULTRA
extruded polystyrene foam boards produced by RBS.
The EPD applies to 1 m3 of XPS board,
with an average density of 41.9 kg/m3.
This declaration is based on the product Scope:
category rules: The data have been provided by the three ISO 14001
Insulating materials made of foam plastics, 01.2019 certified factories of Ravago Building Solutions
(PCR checked and approved by the SVR) producing these products in France, Germany and the
UK for the year 2020.
Issue date
04.01.2023 The owner of the declaration shall be liable for the
underlying information and evidence; the IBU shall not
be liable with respect to manufacturer information, life
Valid to
cycle assessment data and evidences.
03.01.2028
The EPD was created according to the specifications
of EN 15804+A2. In the following, the standard will be
simplified as EN 15804.
Verification
The standard EN 15804 serves as the core PCR
Independent verification of the declaration and data
according to ISO 14025:2011
Dipl. Ing. Hans Peters internally x externally
(chairman of Institut Bauen und Umwelt e.V.)
Dr. Alexander Röder Dr.-Ing. Andreas Ciroth
(Managing Director Institut Bauen und Umwelt e.V.)) (Independent verifier)
Product
Product description/Product definition Trade Association (EU/EFTA) (with the exception of
Switzerland) Regulation (EU) No. 305/2011 (CPR)
RAVATHERM(TM) XPS PLUS, XPS X PLUS and XPS applies. The product needs a declaration of
X ULTRA extruded polystyrene foams (XPS) are performance taking into consideration the EN XPS
thermoplastic insulation foams produced according to standards (EN 13164/ Building insulation,
/EN 13164/ Building insulation, /EN 14307/ Equipment EN 14307 Equipment insulation). For the application
insulation. and use the respective national provisions apply.
They are available in board shape with a density range
from 25 to 50 kg/m3. The boards can be delivered in Application
various compressive strength values from 150 to 700 The variety of the performance properties of
kPa. To meet the need of various applications the RAVATHERM XPS PLUS, X PLUS and X ULTRA
boards are produced with different surfaces: with the thermal insulation foams make them suitable for use in
extrusion skin, planed, grooved or with thermal a large number of applications such as: perimeter
embossing. These XPS boards are supplied with insulation, inverted insulation for terrace roofs,
different edge treatments such as butt edge, ship lap insulation of pitched roofs, floor insulation including
and tongue and groove. The EPD is related to unfaced insulation of highly loaded industrial floors, insulation of
XPS products only; Heat lamination of several XPS thermal bridges for exterior walls, External Thermal
layers is included. Additional product treatment is not Insulation Composite System (ETICS), insulation of
considered. cavity walls, agricultural building ceiling insulation,
prefabricated elements e.g. building sandwich panels,
For the placing on the market of the construction insulation for building equipment and
product in the European Union/ European Free industrial installations (pipe sections, …).
2 Environmental Product Declaration Ravago Building Solutions – RAVATHERM XPS (X) PLUS/ULTRA
altogether up to 8.5% by weight in relation to the
material input.
Technical Data
Acoustic properties are not relevant for XPS foams.
For fire performance these products usually achieve Basic material Mass portion
the fire classification Euroclass E according to /EN Polystyrene 87 - 90 %
13501-1/. Blowing agents 8 - 10 %
HFO-1234ze ~ 60 %
Constructional data CO2, and Co-blowing Agents ~ 40 %
Name Value Unit Flame retardant < 2 %
Gross density 25 - 50 kg/m3 Colorant < 2 %
Compressive strength acc. to EN Additives (e.g. process aid) < 1 %
0.3 - 0.7 N/mm2
826
Tensile strength acc. to EN 826 0.2 - 1.2 N/mm2 Information that the product does not contain
Modulus of elasticity acc. to EN substances listed in the Candidate List of substances
20 - 50 N/mm2
826 of very high concern (/REACH/ Regulation) exceeding
Calculation value for thermal 0.1%:
0.027 -
conductivity /EN 12667/ and /EN W/(mK) This product contains substances listed in the
0.03
13164/ Annex C candidate list (date:17.01.2022) exceeding 0.1
Water vapour diffusion resistance percentage by mass: no
150 -
factor acc. to EN 12088
Creep behaviour or permanent This product contains other Carcinogenic, Mutagenic,
compressive strength acc. to DIN 0.25 N/mm2 Reptrotoxic (CMR) substances in categories 1A or 1B
EN 1606 which are not on the candidate list, exceeding 0.1
percentage by mass: no
Water absorption after diffusion
1 - 3 Vol.-%
acc. to EN 12088
Biocide products were added to this construction
product or it has been treated with biocide products
(this then concerns a treated product as defined by the
Performance data of the product in accordance with
(EU) Ordinance on Biocide Products No. 528/2012): no
the declaration of performance with respect to its
essential characteristics according to /EN
13164:2012+A1:2015/ - Thermal Insulation products
Reference service life
for buildings / /EN 14307:2015/ Thermal Insulation
The durability of XPS foam is normally at least as long
products for building equipment and industrial
as the lifetime of the building/equipment in/with which it
installations.
is used or at least 50 years. This is explained by the
superior mechanical and water resistance properties of
Base materials/Ancillary materials
these products.
RAVATHERMTM XPS (X) PLUS and ULTRA are
mostly made of polystyrene (CAS 9003-53-6), blown
with fluorinated olefin HFO-1234ze (CAS 29118-24-9),
carbon dioxide and halogen-free co-blowing agents
LCA: Calculation rules
Declared Unit environmental impacts may be calculated by linear
The declared unit is 1 m³ of the XPS insulation scaling using the following formular.
product.
The declared product reflects the average of three of
Ravago's sites weighted by production volumes share:
- Rheinmuenster (DE): 43.80 kg/m3 (60%)
- King's Lynn (UK): 40.77 kg/m3 (24%)
- Artix (FR): 36.36 kg/m3 (16%) I adap – adapted LCIA indicator or LCI parameter
I – LCIA indicator or LCI parameter for reference
ref
The weighted average density of the product is 41.9 density of 41.9 kg/m³
kg/m³. p adap – adapted density
p – reference density of 41.9 kg/m³
ref
Corresponding conversion factors are listed in the d adap – adapted board thickness
table below. d ref – thickness of reference board
Declared unit System boundary
Name Value Unit Type of EPD according to EN 15804: "cradle to gate
Declared unit 1 m3 with options, modules C1–C4, and module D". The
Gross density 41.9 kg/m3 following modules are declared: A1–A3, C, D and
additional modules: A4 + A5.
For XPS products with densities or thickness different
from the reference density of 41.9 kg/m³, the Production - Modules A1-A3
The product stage includes:
 Raw material supply (A1)
3 Environmental Product Declaration Ravago Building Solutions – RAVATHERM XPS (X) PLUS/ULTRA
 Transport to the manufacturer (A2): Transport  Transport to EoL (C2)
is considered for up to 92% of the input raw  Waste processing & disposal (C) with two 100
materials % scenarios (scenario 1: thermal treatment
 Manufacturing (A3), including provision of all (C3 and D); scenario 2: landfill (C4))
materials, products and energy, as well as  Reuse, recovery or recycling potential (D) -
waste processing up to the end-of waste beyond system boundary.
state.
Construction stage - Modules A4-A5
The construction process stage includes: Comparability
 Transport to the construction site (A4) Basically, a comparison or an evaluation of EPD data
is only possible if all the data sets to be compared
 Treatment of packaging material (A5)
were created according to EN 15804 and the building
context, respectively the product-specific
End-of-life stage– Modules C1-C4 and D characteristics of performance, are taken into account.
The end-of-life stage includes
 Manual dismantling (C1) Background database: GaBi ts, CUP2021.2
LCA: Scenarios and additional technical information
Characteristic product properties XPS results in benefits, beyond the system boundary,
Information on biogenic carbon for thermal energy and electricity under European
conditions.
Information on describing the biogenic Carbon The transport to End of Life (C2) is calculated with a
Content at factury gate distance of 50 km (with 70% utilization).
Name Value Unit Name Value Unit
Biogenic carbon content in product 0 kg C Collected separately XPS 41.9 kg
Biogenic carbon content in Energy recovery (scenario 1) 41.9 kg
0 kg C
accompanying packaging Landfilling (scenario 2) 41.9 kg
Reuse, recovery and/or recycling potentials (D),
The following technical scenario information is required relevant scenario information
for the declared modules and optional for non-declared
modules. Module D includes the credits of the thermal and
The following technical information is a basis for the electrical energy generated in Module A5 and C3 due
declared modules or can be used for developing to thermal treatment of packaging and product waste
specific scenarios in the context of a building (XPS product).
assessment if modules are not declared (MND). The
values refer to the declared unit of 1 m3 XPS product. Avoided burdens have been calculated by the
inversion of residual grid mix and thermal energy from
Transport to the building site (A4) natural gas, using European datasets.
Name Value Unit
Payload of truck 5 t A waste incineration plant with R1-value > 0.6 is
Transport distance (weighted average assumed.
476 km
based on production volumes)
Capacity utilisation (including empty
70 %
runs)
Gross density of products transported 41.9 kg/m3
The transport distance can be modified to project-
specific criteria if required by linear scaling.
Installation into the building (A5)
The thermal treatment of the packaging is considered
here. The following quantities are produced per m3 of
XPS product:
Name Value Unit
LDPE packaging film (weighted
average based on production volume 0.671 kg
shares)
End of life (C1-C4)
For the End of Life stage two different scenarios are
considered. One scenario with 100% incineration
(scenario 1: C3, D) and one scenario with 100% landfill
(senario. 2: C4) are calculated. The incineration of
4 Environmental Product Declaration Ravago Building Solutions – RAVATHERM XPS (X) PLUS/ULTRA
LCA: Results
The following tables display the environmental relevant results according to /EN 15804/ for 1 m3 XPS board. The
two EoL Scenarios are represented in modules C3/1, C4/2, D/1, and D/2. C3/1 and D/1 show the environmental
results in case of thermal treatment of XPS product. D/1 covers also the results of the packaging treatment from
Module A5. Module C4/2 reflects the landfilling of XPS (for scenario 2 "landfilling" the values in Module D for XPS
are 0). Hence. Module D/2 shows only the environmental results of the packaging treatment from module A5.
DESCRIPTION OF THE SYSTEM BOUNDARY (X = INCLUDED IN LCA; ND = MODULE OR INDICATOR NOT
DECLARED; MNR = MODULE NOT RELEVANT)
BENEFITS AND
CONSTRUCTI LOADS
PRODUCT STAGE ON PROCESS USE STAGE END OF LIFE STAGE BEYOND THE
STAGE SYSTEM
BOUNDARIES
5 Environmental Product Declaration Ravago Building Solutions – RAVATHERM XPS (X) PLUS/ULTRA
lairetam
waR
ylppus tropsnarT
gnirutcafunaM
eht
morf
tropsnarT
etis
eht
ot
etag
ylbmessA esU
ecnanetniaM
riapeR
tnemecalpeR tnemhsibrufeR
ygrene
lanoitarepO esu
retaw
lanoitarepO esu
noitcurtsnoc-eD
noitilomed tropsnarT
gnissecorp
etsaW
lasopsiD -esueR -yrevoceR -gnilcyceR laitnetop
A1 A2 A3 A4 A5 B1 B2 B3 B4 B5 B6 B7 C1 C2 C3 C4 D
X X X X X ND ND MNR MNR MNR ND ND X X X X X
RESULTS OF THE LCA - ENVIRONMENTAL IMPACT according to EN 15804+A2: 1 m3 XPS product
Core Indicator Unit A1-A3 A4 A5 C1 C2 C3/1 C4/2 D/1 D/2
GWP-total [kg CO2-Eq.] 1.30E+2 3.26E+0 2.10E+0 0.00E+0 3.36E-1 1.40E+2 2.97E+0 -5.99E+1 -1.09E+0
GWP-fossil [kg CO2-Eq.] 1.29E+2 3.23E+0 2.10E+0 0.00E+0 3.34E-1 1.40E+2 3.00E+0 -5.96E+1 -1.09E+0
GWP-biogenic [kg CO2-Eq.] 4.75E-1 -4.15E-3 6.96E-5 0.00E+0 -4.28E-4 4.35E-3 -3.13E-2 -2.95E-1 -1.29E-3
GWP-luluc [kg CO2-Eq.] 3.78E-2 2.67E-2 1.12E-5 0.00E+0 2.75E-3 7.72E-4 2.51E-3 -4.09E-2 -1.13E-4
ODP [kg CFC11-Eq.] 4.04E-13 4.16E-16 1.57E-16 0.00E+0 4.29E-17 1.02E-14 7.24E-15 -6.80E-13 -6.23E-15
AP [mol H+-Eq.] 2.62E-1 1.01E-2 2.09E-4 0.00E+0 1.04E-3 1.24E-2 8.99E-3 -7.80E-2 -1.21E-3
EP-freshwater [kg P-Eq.] 1.49E-4 9.66E-6 2.10E-8 0.00E+0 9.97E-7 1.38E-6 5.54E-4 -7.73E-5 -2.53E-7
EP-marine [kg N-Eq.] 5.97E-2 4.63E-3 4.39E-5 0.00E+0 4.78E-4 2.74E-3 2.04E-3 -2.22E-2 -3.75E-4
EP-terrestrial [mol N-Eq.] 6.52E-1 5.19E-2 9.80E-4 0.00E+0 5.35E-3 5.82E-2 2.24E-2 -2.37E-1 -4.06E-3
POCP [kg NMVOC-Eq.] 6.98E-1 9.07E-3 1.31E-4 0.00E+0 9.36E-4 8.06E-3 6.52E-3 -6.22E-2 -1.08E-3
ADPE [kg Sb-Eq.] 1.29E-5 2.48E-7 2.37E-9 0.00E+0 2.56E-8 1.54E-7 2.06E-7 -9.88E-6 -9.51E-8
ADPF [MJ] 3.76E+3 4.33E+1 2.56E-1 0.00E+0 4.47E+0 1.63E+1 4.38E+1 -1.04E+3 -2.05E+1
[m³ world-Eq
WDP 2.23E+1 2.83E-2 1.93E-1 0.00E+0 2.92E-3 1.14E+1 -3.70E-2 -4.56E+0 -4.44E-2
deprived]
GWP = Global warming potential; ODP = Depletion potential of the stratospheric ozone layer; AP = Acidification potential of land and water; EP =
Caption Eutrophication potential; POCP = Formation potential of tropospheric ozone photochemical oxidants; ADPE = Abiotic depletion potential for non-
fossil resources; ADPF = Abiotic depletion potential for fossil resources; WDP = Water (user) deprivation potential
RESULTS OF THE LCA - INDICATORS TO DESCRIBE RESOURCE USE according to EN 15804+A2: 1 m3
XPS product
Indicator Unit A1-A3 A4 A5 C1 C2 C3/1 C4/2 D/1 D/2
PERE [MJ] 1.14E+2 2.42E+0 5.06E-2 0.00E+0 2.49E-1 3.27E+0 3.18E+0 -2.33E+2 -1.20E+0
PERM [MJ] 0.00E+0 0.00E+0 0.00E+0 0.00E+0 0.00E+0 0.00E+0 0.00E+0 0.00E+0 0.00E+0
PERT [MJ] 1.14E+2 2.42E+0 5.06E-2 0.00E+0 2.49E-1 3.27E+0 3.18E+0 -2.33E+2 -1.20E+0
PENRE [MJ] 2.06E+3 4.34E+1 3.11E+1 0.00E+0 4.48E+0 1.69E+3 4.38E+1 -1.04E+3 -2.05E+1
PENRM [MJ] 1.71E+3 0.00E+0 -3.09E+1 0.00E+0 0.00E+0 -1.68E+3 0.00E+0 0.00E+0 0.00E+0
PENRT [MJ] 3.77E+3 4.34E+1 2.56E-1 0.00E+0 4.48E+0 1.63E+1 4.38E+1 -1.04E+3 -2.05E+1
SM [kg] 0.00E+0 0.00E+0 0.00E+0 0.00E+0 0.00E+0 0.00E+0 0.00E+0 0.00E+0 0.00E+0
RSF [MJ] 0.00E+0 0.00E+0 0.00E+0 0.00E+0 0.00E+0 0.00E+0 0.00E+0 0.00E+0 0.00E+0
NRSF [MJ] 0.00E+0 0.00E+0 0.00E+0 0.00E+0 0.00E+0 0.00E+0 0.00E+0 0.00E+0 0.00E+0
FW [m³] 6.33E-1 2.77E-3 4.52E-3 0.00E+0 2.86E-4 2.68E-1 4.03E-4 -2.29E-1 -2.61E-3
PERE = Use of renewable primary energy excluding renewable primary energy resources used as raw materials; PERM = Use of
renewable primary energy resources used as raw materials; PERT = Total use of renewable primary energy resources; PENRE = Use of
non-renewable primary energy excluding non-renewable primary energy resources used as raw materials; PENRM = Use of non-
Caption
renewable primary energy resources used as raw materials; PENRT = Total use of non-renewable primary energy resources; SM = Use
of secondary material; RSF = Use of renewable secondary fuels; NRSF = Use of non-renewable secondary fuels; FW = Use of net fresh
water
RESULTS OF THE LCA – WASTE CATEGORIES AND OUTPUT FLOWS according to EN 15804+A2:
1 m3 XPS product
Indicator Unit A1-A3 A4 A5 C1 C2 C3/1 C4/2 D/1 D/2
HWD [kg] 2.92E-7 2.19E-9 4.56E-11 0.00E+0 2.26E-10 2.92E-9 7.87E-9 -2.32E-7 -3.07E-9
NHWD [kg] 9.87E-1 6.44E-3 8.30E-3 0.00E+0 6.65E-4 8.06E-1 4.17E+1 -4.83E-1 -4.33E-3
RWD [kg] 7.89E-2 5.25E-5 1.45E-5 0.00E+0 5.41E-6 9.24E-4 5.08E-4 -7.63E-2 -1.85E-3
CRU [kg] 0.00E+0 0.00E+0 0.00E+0 0.00E+0 0.00E+0 0.00E+0 0.00E+0 0.00E+0 0.00E+0
MFR [kg] 0.00E+0 0.00E+0 0.00E+0 0.00E+0 0.00E+0 0.00E+0 0.00E+0 0.00E+0 0.00E+0
MER [kg] 0.00E+0 0.00E+0 0.00E+0 0.00E+0 0.00E+0 0.00E+0 0.00E+0 0.00E+0 0.00E+0
EEE [MJ] 0.00E+0 0.00E+0 4.47E+0 0.00E+0 0.00E+0 2.54E+2 0.00E+0 0.00E+0 0.00E+0
EET [MJ] 0.00E+0 0.00E+0 7.95E+0 0.00E+0 0.00E+0 4.53E+2 0.00E+0 0.00E+0 0.00E+0
HWD = Hazardous waste disposed; NHWD = Non-hazardous waste disposed; RWD = Radioactive waste disposed; CRU = Components
Caption for re-use; MFR = Materials for recycling; MER = Materials for energy recovery; EEE = Exported electrical energy; EET = Exported
thermal energy
RESULTS OF THE LCA – additional impact categories according to EN 15804+A2-optional:
1 m3 XPS product
Indicator Unit A1-A3 A4 A5 C1 C2 C3/1 C4/2 D/1 D/2
[Disease
PM 2.16E-6 5.40E-8 1.24E-9 0.00E+0 5.57E-9 7.31E-8 8.81E-8 -6.71E-7 -1.11E-8
Incidence]
[kBq U235-
IRP 1.18E+1 7.51E-3 2.31E-3 0.00E+0 7.75E-4 1.46E-1 7.29E-2 -1.25E+1 -2.70E-1
Eq.]
ETP-fw [CTUe] 2.09E+3 3.13E+1 1.16E-1 0.00E+0 3.23E+0 7.83E+0 4.16E+1 -2.18E+2 -3.58E+0
HTP-c [CTUh] 4.23E-8 6.32E-10 1.34E-11 0.00E+0 6.52E-11 7.75E-10 1.86E-9 -9.82E-9 -1.24E-10
HTP-nc [CTUh] 1.76E-6 3.70E-8 4.24E-10 0.00E+0 3.82E-9 2.55E-8 1.56E-7 -3.88E-7 -6.01E-9
SQP [-] 8.08E+1 1.49E+1 7.17E-2 0.00E+0 1.54E+0 4.59E+0 2.98E+0 -1.59E+2 -9.63E-1
PM = Potential incidence of disease due to PM emissions; IR = Potential Human exposure efficiency relative to U235; ETP-fw = Potential
Caption comparative Toxic Unit for ecosystems; HTP-c = Potential comparative Toxic Unit for humans (cancerogenic); HTP-nc = Potential
comparative Toxic Unit for humans (not cancerogenic); SQP = Potential soil quality index
Disclaimer 1 – for the indicator “Potential Human exposure efficiency relative to U235”.
This impact category deals mainly with the eventual impact of low dose ionizing
radiation on human health of the nuclear fuel cycle. It does not consider effects due to possible
nuclear accidents, occupational exposure nor due to radioactive waste disposal in underground
facilities. Potential ionizing radiation from the soil, from radon and from some construction materials is also not
measured by this indicator.
Disclaimer 2 – for the indicators “abiotic depletion potential for non-fossil resources”, “abiotic depletion potential
for fossil resources”, “water (user) deprivation potential, deprivation-weighted water consumption”, “potential
comparative toxic unit for ecosystems”, “potential comparative toxic unit for humans – cancerogenic”, “Potential
comparative toxic unit for humans - not cancerogenic”, “potential soil quality index”.
The results of this environmental impact indicator shall be used with care as the
uncertainties on these results are high or as there is limited experienced with the indicator.
References
EN 13164 + A1
EN 13164:2012 + A1:2015 Thermal insulation products
for buildings - Factory-made extruded polystyrene ISO 14025
foam (XPS) products - Specification DIN EN ISO 14025:2011-10, Environmental labels and
declarations — Type III environmental declarations —
EN 14307 Principles and procedures.
EN 14307:2015 Thermal insulation products for
building equipment and industrial installations - IBU 2021
Factory-made extruded polystyrene foam (XPS) Institut Bauen und Umwelt e.V.: General Instructions
products - Specification for the EPD programme of Institut Bauen und Umwelt
e.V., Version 2.0, Berlin: Institut Bauen und Umwelt
EN 12667 e.V., 2021
EN 12667:2001 Thermal performance of building www.ibu-epd.com
materials and products - Determination of thermal /CPR/
resistance by means of guarded hot plate and heat Regulation No. 305/2011: Construction Products
flow meter methods - Products of high and medium Regulation of the European Parliament and of the
thermal resistance European Council, 2011.
EN 13501 /PCR Part A/
EN 13501-1:2019-05 Fire classification of construction PCR - Part A: Calculation rules for the Life Cycle
products and building elements - Part 1: Classification Assessment and Requirements on the Background
using data from reaction to fire tests Report, version 2.1, Institut Bauen und Umwelt e.V.,
2021, www.bau-umwelt.com
EN 15804 /PCR Part B/
EN 15804+A2:2019+AC:2021 (in press), Sustainability PCR – Part B: Requirements of the EPD for Insulating
of construction works — Environmental Product materials made of foam plastics, version 1.7, 2019,
Declarations — Core rules for the product category of Institut Bauen und Umwelt e.V., www.bau-umwelt.com
construction products.
6 Environmental Product Declaration Ravago Building Solutions – RAVATHERM XPS (X) PLUS/ULTRA
Publisher
Institut Bauen und Umwelt e.V. Tel +49 (0)30 3087748- 0
Hegelplatz 1 Fax +49 (0)30 3087748- 29
10117 Berlin Mail info@ibu-epd.com
Germany Web www.ibu-epd.com
Programme holder
Institut Bauen und Umwelt e.V. Tel +49 (0)30 - 3087748- 0
Hegelplatz 1 Fax +49 (0)30 – 3087748 - 29
10117 Berlin Mail info@ibu-epd.com
Germany Web www.ibu-epd.com
Author of the Life Cycle
Assessment Tel +49 711 341817-0
Sphera Solutions GmbH Fax +49 711 341817-25
Hauptstraße 111- 113 Mail info@sphera.com
70771 Leinfelden-Echterdingen Web www.sphera.com
Germany
Owner of the Declaration
Ravago Building Solutions Tel none
Germany GmbH Fax none
Value Park Y51 Mail info.industry.rbs@ravago.com
06258 Schkopau Web
Germany www.ravagobuildingsolutions.
com/industry
