Environmental Product Declaration (EPD)
According to ISO 14025 and EN 15804
reinforcing stabilized
three and seven-wire
strands with and
without dents with a
nominal tensile
strength of 1670÷1860
N /mm2 with a
diameter of 6.5÷15.7
mm (PC-strand) .
Registration number: EPD-Kiwa-EE-162692-EN
Issue date: 21-12-2023
Valid until: 21-12-2028
Declaration owner: PJSC "STALKANAT"
Publisher: Kiwa-Ecobility Experts
Program operator: Kiwa-Ecobility Experts
Status: verified
reinforcing stabilized three and seven-wire strands with and without dents with a nominal tensile strength of 1670÷1860 N /mm2 with a diameter of 6.5÷15.7 mm (PC-strand) . | ReTHiNK-62692 1 / 17
Environmental Product Declaration
1 General information
E-mail: gremecheva_sb@stalkanat.com.ua
1.1 PRODUCT Website: https://stalkanat.com.ua/
Production location: PJSC " Stalkanat"
reinforcing stabilized three and seven-wire strands with and without dents with a nominal
tensile strength of 1670÷1860 N /mm2 with a diameter of 6.5÷15.7 mm (PC-strand) . Address production location: Vapnyana St, 52A, 65006 Odessa, UA
1.2 REGISTRATION NUMBER 1.6 VERIFICATION OF THE DECLARATION
EPD-Kiwa-EE-162692-EN
The independent verification is in accordance with the ISO 14025:2011. The LCA is in
compliance with ISO 14040:2006 and ISO 14044:2006. The EN 15804:2012+A2:2019 serves as
1.3 VALIDITY
the core PCR.
Issue date: 21-12-2023 Internal ✓ External
Valid until: 21-12-2028
1.4 PROGRAM OPERATOR
Kiwa-Ecobility Experts
Voltastraße 5
13355 Berlin
DE Anne Kees Jeeninga, Advieslab
1.7 STATEMENTS
The owner of this EPD shall be liable for the underlying information and evidence. The
Prof. Dr. Frank Heimbecher
programme operator Kiwa-Ecobility Experts shall not be liable with respect to
manufacturer data, life cycle assessment data and evidence.
(Chairman of the independent expert
committee - Kiwa-Ecobility Experts)
1.8 PRODUCT CATEGORY RULES
Frank Huppertz
PCR A
PCR A – General Program Category Rules for Construction Products from the EPD
(Head of Kiwa-Ecobility Experts)
programme of Kiwa-Ecobility Experts; Version 2.1 (2022)
PCR B
1.5 OWNER OF THE DECLARATION
Kiwa-Ecobility Experts, Berlin, 2020: PCR B – Product Category Rules for steel construction
products, Requirements on the Environmental Product Declarations for steel construction
Manufacturer: PJSC "STALKANAT" products; Version 2020-03-13 (draft)
Address: str. Vodoprovidna 16,, 65007 Odesa, UA
reinforcing stabilized three and seven-wire strands with and without dents with a nominal tensile strength of 1670÷1860 N /mm2 with a diameter of 6.5÷15.7 mm (PC-strand) . | ReTHiNK-62692 2 / 17
Environmental Product Declaration
1 General information
Characterization method: EN 15804 +A2 Method v1.0
1.9 COMPARABILITY LCA database profiles: EcoInvent version 3.6
Version database: v3.15 (2023-07-12)
In principle, a comparison or assessment of the environmental impacts of different
products is only possible if they have been prepared in accordance with EN 15804. For the
* Used for calculating the characterized results of the Environmental profiles within
evaluation of the comparability, the following aspects have to be considered in particular:
R<THiNK.
PCR used, functional or declared unit, geographical reference, the definition of the system
boundary, declared modules, data selection (primary or secondary data, background
database, data quality), scenarios used for use and disposal phases, and the life cycle 1.11 LCA BACKGROUND REPORT
inventory (data collection, calculation methods, allocations, validity period). PCRs and
general program instructions of different EPDs programs may differ. Comparability needs This EPD is generated on the basis of the LCA background report 'reinforcing stabilized
to be evaluated. For further guidance, see EN 15804+A2 (5.3 Comparability of EPD for three and seven-wire strands with and without dents with a nominal tensile strength of
construction products) and ISO 14025 (6.7.2 Requirements for comparability). 1670÷1860 N /mm2 with a diameter of 6.5÷15.7 mm (PC-strand) .' with the calculation
identifier ReTHiNK-62692.
1.10 CALCULATION BASIS
LCA method R<THiNK: Ecobility Experts | EN15804+A2
LCA software*: Simapro 9.1
reinforcing stabilized three and seven-wire strands with and without dents with a nominal tensile strength of 1670÷1860 N /mm2 with a diameter of 6.5÷15.7 mm (PC-strand) . | ReTHiNK-62692 3 / 17
Environmental Product Declaration
2 Product
2.1 PRODUCT DESCRIPTION
Product type according to REACH No. 1907/2006 – construction product. It is not classified
as a hazardous substance. Conditions for safe storage, including any incompatibilities:
This EPD applies to steel reinforcing stabilized three and seven-wire strands with or
Avoid moisture, acids and other factors that may corrode the metal. When warehousing
without dents with a nominal tensile strength of 1670÷1860 N/mm2 with the diameter of
and storing, keep the original packaging.
6.5÷15.7 mm, produced by PJSC "STALKANAT".
Information on toxicological effects: The product has no toxicological effects.
The investigated product - PC-strand reinforcing strands is a twisted product of three or
seven wires twisted together around a common axis. After laying on a cable machine, the
strands are subjected to thermomechanical treatment (heating and stretching) to stabilize
the mechanical properties.
Reinforcing strands are mainly used for the manufacture of precast concrete elements,
hollow core slabs, beams, TT slabs or railway sleepers, as well as in post-tensioned
structures such as bridges, viaducts or silos. For transportation and storage, the strands are
wound into coils with in-line (precision) laying of the following sizes:
- outer diameter of the coil - no more than 1600 mm;
- inner diameter of the coil - 750 mm, 800 mm, 900 mm;
- bay width - 750 mm, 630 mm.
- weight (1 - 4) tons.
All reinforcing strands can be made from both smooth wire and dented wire. The standard
tensile strength is 1860 MPa, but other strengths are available. Three-wire strands are
twisted from wire of the same diameter. In seven-wire strands, the diameter of the center
wire is at least 3% larger than that of the outer spiral wire. The standard geometric and 2.2 APPLICATION (INTENDED USE OF THE PRODUCT)
mechanical properties of each bundle of strands are tested and verified in our own
laboratory as well as in independent accredited laboratories in accordance with EN ISO Reinforcing strands are mainly used for the manufacture of precast concrete elements,
15630-3. They are also constantly monitored by the relevant certification bodies, ensuring hollow core slabs, beams, TT slabs or railway sleepers, as well as in post-tensioned
full compliance with product standards. structures such as bridges, viaducts or silos. For transportation and storage, the strands are
wound into coils with in-line (precision) laying of the following sizes:
The strands are wound into coils, which are tied with a metal tape 0.8x32 mm in 8 places
evenly spaced around the skein. - outer diameter of the coil - no more than 1600 mm;
The strands are packed in polypropylene fabric. Packaging should protect the strand from - inner diameter of the coil - 750 mm, 800 mm, 900 mm;
mechanical damage and corrosion during transportation and storage.
- bay width - 750 mm, 630 mm.
After packing, the skein of strands is tied to wooden bars with a steel strap for easy
transportation. - weight (1 ÷ 4) tons.
In standard environmental conditions, steel strands represent a stable product, devoid of
any fire or explosion risks. However, it's crucial to note that polypropylene packaging fabric
and wooden blocks, employed for stowage in vehicles during transportation to consumers,
are susceptible to ignition in the presence of open flames. To mitigate this risk, it is
imperative to exercise precautions. Specifically, during the storage and transportation
phases, ensure a considerable distance from potential sources of ignition.
reinforcing stabilized three and seven-wire strands with and without dents with a nominal tensile strength of 1670÷1860 N /mm2 with a diameter of 6.5÷15.7 mm (PC-strand) . | ReTHiNK-62692 4 / 17
Environmental Product Declaration
2 Product
2.3 REFERENCE SERVICE LIFE the references section of this EPD) that are manufactured via the blast furnace/basic
oxygen furnace route (BF/BOF), followed by hot rolling.) used as raw material and auxiliary
products that are used at each stage of the process.
RSL PRODUCT
Since the service life of wire strands is not considered, there is no need to specify a The production process consists of the following production steps:
reference service life. The generic life cycle of product can be considered as 100 years for
any calculations basics. - Removal of scale mechanically. Hot rolled products have a layer of iron oxides on
their surface, which must be removed before drawing. This process is carried out on a
USED RSL (YR) IN THIS LCA CALCULATION: surface preparation line installed in front of the drawing bench. The wire rod passes
through the steel rollers, bends on them, the scale falls off the surface of the wire rod. After
100
removing the scale in the rollers, the surface of the wire rod is treated with rotating steel
brushes to remove any remaining scale. Then the wire rod is washed with water, coated
2.4 TECHNICAL DATA with products (phosphate + borax) that promote lubrication at the next stage of wire
drawing. Before drawing, the wire rod is dried with hot air.
In particular, the manufacturer declares the following information about the technical
- Wire drawing. In cold drawing, the wire rod is passed through several consecutive
characteristics of the product:
drawing dies installed on the drawing bench, which leads to a decrease in the cross
section and a change in physical characteristics. To facilitate passage through the dies,
Tensile modulus
powdered soaps are used to reduce the friction of the wire in the dies. When the wire rod
195 GPa ± 10% (strand) passes through successive dies, the cross section is reduced to a given size, the material is
also strengthened and the surface of the wire is smooth.
Elongation ≥ 3.5% at L ≥ 500 mm
- Applying dents. To improve adhesion to concrete, the wire is passed through
Low relaxation ≤ 2.5% after 1,000 hours of stress with a load of 70% of the breaking force. pinch rollers mounted on the drawing bench after the last die.
A nominal tensile strength of 1670÷1860 N/mm2 with the diameter of D=4,85÷15,7 mm. - Twisting. In this step, the wires are helically twisted into a strand in a rebar strand
production line to form different types of strands.
PJSC «Stalkanat» produces strands for the European Union according to the following
standards: FprEN 10138-1,3:2009, prEN 10138 –1,3:2006, prEN 10138-1,3:2011, SFS 1265-1,3:2014, - Stabilization. To eliminate the stresses in the wire that occur during the drawing
SS 212551:2013, SS 212553:2013, АТ 001SC-01/314-2023, GOST 13840-68, BS 5896:2012, ÖNORM process, the strands are thermomechanically treated under specified temperature
B 4758:2014, NMÉ: A-16/2018, NMÉ: A-27/2019, NEN 3868:2001, SI 1735, Part 4, ITB- conditions and tension, subsequently the strand is cooled with water at a controlled
KOT-2018/0637, NEN 3868:2001. temperature, and finally air dried to prevent wetting and rusting of the strand.
- Winding. Reinforcing strands are wound into coils for shipment to the consumer.
2.5 DESCRIPTION PRODUCTION PROCESS
- Package. Coils of strands are packed in polypropylene fabric.
The rebar plant receives the components necessary for the production of products: wire
rod (Carbon steel reinforcing bars (“rebar”) (according to the product standards listed in
reinforcing stabilized three and seven-wire strands with and without dents with a nominal tensile strength of 1670÷1860 N /mm2 with a diameter of 6.5÷15.7 mm (PC-strand) . | ReTHiNK-62692 5 / 17
Environmental Product Declaration
3 Calculation rules
3.1 DECLARED UNIT Module D = Benefits and loads beyond the
Module B3 = Repair
product system boundaries
Kg
Module B4 = Replacement
The declared functional unit is 1 kg. Other declared units are permissible if conversion to 1
kg is depicted in a transparent manner.
3.4 REPRESENTATIVENESS
reference_unit: kilogram (kg)
This EPD is representative for reinforcing stabilized three and seven-wire strands with and
3.2 CONVERSION FACTORS without dents with a nominal tensile strength of 1670÷1860 N /mm2 with a diameter of
6.5÷15.7 mm (PC-strand) ., a product of PJSC "STALKANAT". The results of this EPD are
representative for European Union.
Description Value Unit
reference_unit 1 kg
3.5 CUT-OFF CRITERIA
Conversion factor to 1 kg 1.000000 kg
Product Stage (A1-A3)
3.3 SCOPE OF DECLARATION AND SYSTEM BOUNDARIES
The production stage encompasses the transportation of raw materials, the conversion of
these raw materials(steel Purchased from the steel supplier) into the end product. This
This is a Cradle to gate with modules C1-C4 and module D LCA. The life cycle stages
phase accounts for the energy necessary for production, supplementary materials,
included are as shown below: packaging materials, and the associated emissions. It's important to note that certain
processes, such as wire drawing, and emissions generated therein, are excluded from
(X = module included, ND = module not declared)
consideration, as their impact is minimal, constituting less than 1% of the overall steel
A1 A2 A3 A4 A5 B1 B2 B3 B4 B5 B6 B7 C1 C2 C3 C4 D impact. Therefore, the analysis primarily focuses on electricity consumption and input
materials.
X X X ND ND ND ND ND ND ND ND ND X X X X X
Construction process stage (A4-A5)
The modules of the EN15804 contain the following:
Module A1 = Raw material supply Module B5 = Refurbishment This stage consists the transport of the product from production plant to the construction
site.
Module A2 = Transport Module B6 = Operational energy use
Module A3 = Manufacturing Module B7 = Operational water use It also includes the loss of material during construction. The additional needed production,
transport and end-of-life of the lost material during construction is included.
Module A4 = Transport Module C1 = De-construction / Demolition
The end-of-life of packaging material up to the end-of-waste state or disposal of final
Module A5 = Construction -
Module C2 = Transport residues is also included.
Installation process
Module B1 = Use Module C3 = Waste Processing
Use stage (B1-B3)
Module B2 = Maintenance Module C4 = Disposal
reinforcing stabilized three and seven-wire strands with and without dents with a nominal tensile strength of 1670÷1860 N /mm2 with a diameter of 6.5÷15.7 mm (PC-strand) . | ReTHiNK-62692 6 / 17
Environmental Product Declaration
3 Calculation rules
This stage consists of the impacts arising from components of the building and In addition, the benefits of energy recovery are granted at this stage. The amount of avoid
construction works during their use. energy is based on the Lower Heating Values of the materials and the efficiencies of the
incinerators as mentioned in the NMD Determination method v1.0 or EcoInvent 3.6 (2019)
The stage also covers the combination of all planned technical and associated
administrative maintenance actions during the service life to maintain the product In accordance with the criteria of the reference standard, the system has been extended as
installed in a building, in a construction works or its parts in a state in which it can perform far as possible to avoid attributing environmental impacts to by-products of multi-unit
its required functional and technical performance, as well as preserve the aesthetic processes within the manufacturing process.
qualities of the product. This will include preventative and regular maintenance activities.
If necessary, distribution was applied to the inputs and outputs of the system based on
Product replacement (B4) and renovation (B5) only apply when the product is considered physical properties (mass or volume).
in a lifespan (of a building, work , etc.).
There was no need to apply economic criteria.
Operational water and energy use are not considered.
3.6 ALLOCATION
End of life stage (C1-C4)
Allocation were avoided
When the end of the life stage of the building is reached, the de-construction/demolition
begins. This EPD includes de-construction/demolition (C1), the necessary transport (C2) 3.7 DATA COLLECTION & REFERENCE TIME PERIOD
from the demolition site to the sorting location and distance to final disposal. The end of
life stage includes the final disposal to landfill (C4), incineration (C3) and needed recycling 01.01.2022-31.01.2023
processes up to the end-of-waste point (C3). Loads and benefits of recycling, re-use and
exported energy are part of module D.
3.8 ESTIMATES AND ASSUMPTIONS
The prescribed waste scenarios from the NMD Determination method v1.1 have been used
for the various materials in the product. The Purschase of Steel is generalized to 100% from Arcelor as mostly the steel is from
Arcelor and sometimes (only in special cases of non-availability) it is purchased from other
supplier and there is no fixed quantity for same hence, that can be neglected.
Benefits and Loads beyond the system boundary (Module D)
Electricity Mix is used according to the general low voltage electricty mix of Ukraine (local
based approach).
This stage contains the potential loads and benefits of recycling and re-use of raw
materials/products. The loads contain the needed recycling processes from end-of-waste-
point up to the point-of-equivalence of the substituted primary raw material and a load for
secondary material that will be lost at the end-of-life stage.
3.9 DATA QUALITY
The loads and benefits of recycling and reuse are included in this module. The benefits are
calculated based on the primary content and the primary equivalent.
Data quality is as per the data shared by the client with the measured values.
reinforcing stabilized three and seven-wire strands with and without dents with a nominal tensile strength of 1670÷1860 N /mm2 with a diameter of 6.5÷15.7 mm (PC-strand) . | ReTHiNK-62692 7 / 17
Environmental Product Declaration
4 Scenarios and additional technical information
4.1 DE-CONSTRUCTION, DEMOLITION (C1)
No inputs are needed for the product at the de-construction / demolition phase
4.2 TRANSPORT END-OF-LIFE (C2)
The following distances and transport conveyance are assumed for transportation during
end of life for the different types of waste processing.
Waste Scenario Transport conveyance Not removed (stays in work) Landfill Incineration Recycling Re-use
[km] [km] [km] [km] [km]
Steel, reinforcement (NMD ID Lorry (Truck), unspecified (default) | market group for
0 100 150 50 0
74) (GLO)
The transport conveyance(s) used in the scenario(s) for transport during end of life has the
following characteristics.
Value and unit
Vehicle type used for transport Lorry (Truck), unspecified (default) | market group for (GLO)
Fuel type and consumption of vehicle not available
Capacity utilisation (including empty returns) 50 % (loaded up and return empty)
Bulk density of transported products inapplicable
Volume capacity utilisation factor 1
4.3 END OF LIFE (C3, C4)
The scenario(s) assumed for end of life of the product are given in the following tables.
First the assumed percentages per type of waste processing are displayed, followed by the
assumed amounts.
Waste Scenario Region Not removed (stays in work) [%] Landfill [%] Incineration [%] Recycling [%] Re-use [%]
Steel, reinforcement (NMD ID 74) NL 0 5 0 95 0
reinforcing stabilized three and seven-wire strands with and without dents with a nominal tensile strength of 1670÷1860 N /mm2 with a diameter of 6.5÷15.7 mm (PC-strand) . | ReTHiNK-62692 8 / 17
Environmental Product Declaration
4 Scenarios and additional technical information
Waste Scenario Not removed (stays in work) [kg] Landfill [kg] Incineration [kg] Recycling [kg] Re-use [kg]
Steel, reinforcement (NMD ID 74) 0.000 0.050 0.000 0.950 0.000
Total 0.000 0.050 0.000 0.950 0.000
4.4 BENEFITS AND LOADS BEYOND THE SYSTEM BOUNDARY (D)
The presented Benefits and loads beyond the system boundary in this EPD are based on
the following calculated Net output flows in kilograms and Energy recovery displayed in
MJ Lower Heating Value.
Waste Scenario Net output flow [kg] Energy recovery [MJ]
Steel, reinforcement (NMD ID 74) 0.950 0.000
Total 0.950 0.000
reinforcing stabilized three and seven-wire strands with and without dents with a nominal tensile strength of 1670÷1860 N /mm2 with a diameter of 6.5÷15.7 mm (PC-strand) . | ReTHiNK-62692 9 / 17
Environmental Product Declaration
5 Results
For the impact assessment, the characterization factors of the LCIA method EN 15804 +A2
Method v1.0 are used. Long-term emissions (>100 years) are not considered in the impact
assessment. The results of the impact assessment are only relative statements that do not
make any statements about end-points of the impact categories, exceedance of threshold
values, safety margins or risks. The following tables show the results of the indicators of the
impact assessment, of the use of resources as well as of waste and other output flows.
5.1 ENVIRONMENTAL IMPACT INDICATORS PER KILOGRAM
CORE ENVIRONMENTAL IMPACT INDICATORS EN15804+A2
Abbreviation Unit A1 A2 A3 C1 C2 C3 C4 D
AP mol H+ eqv. 2.92E-3 1.92E-4 1.01E-3 0.00E+0 4.11E-5 0.00E+0 2.50E-6 -5.22E-3
GWP-total kg CO2 eqv. 2.54E+0 2.27E-2 2.71E-1 0.00E+0 7.09E-3 0.00E+0 2.64E-4 -1.34E+0
GWP-b kg CO2 eqv. -3.12E-3 1.29E-4 2.83E-3 0.00E+0 3.27E-6 0.00E+0 5.22E-7 1.41E-2
GWP-f kg CO2 eqv. 2.54E+0 2.25E-2 2.60E-1 0.00E+0 7.09E-3 0.00E+0 2.63E-4 -1.35E+0
GWP-luluc kg CO2 eqv. 3.35E-4 2.67E-5 8.14E-3 0.00E+0 2.60E-6 0.00E+0 7.34E-8 9.99E-4
EP-m kg N eqv. 6.15E-3 6.74E-5 3.53E-4 0.00E+0 1.45E-5 0.00E+0 8.60E-7 -9.68E-4
EP-fw kg P eqv. 3.49E+0 9.51E-7 9.36E-2 0.00E+0 7.15E-8 0.00E+0 2.95E-9 -4.78E-5
EP-T mol N eqv. 1.65E-3 7.47E-4 1.62E-3 0.00E+0 1.60E-4 0.00E+0 9.48E-6 -1.13E-2
ODP kg CFC 11 eqv. 2.00E-15 3.08E-9 8.18E-9 0.00E+0 1.56E-9 0.00E+0 1.08E-10 -3.30E-8
kg NMVOC
POCP 1.28E-7 2.03E-4 3.35E-4 0.00E+0 4.56E-5 0.00E+0 2.75E-6 -7.69E-3
eqv.
ADP-f MJ 5.06E+0 3.31E-1 1.86E+0 0.00E+0 1.07E-1 0.00E+0 7.36E-3 -9.45E+0
ADP-mm kg Sb-eqv. 2.60E+1 1.81E-7 6.97E-1 0.00E+0 1.80E-7 0.00E+0 2.41E-9 -9.14E-7
WDP m3 world eqv. 2.78E-8 2.92E-3 6.38E-1 0.00E+0 3.82E-4 0.00E+0 3.30E-4 -2.58E-1
AP=Acidification (AP) | GWP-total=Global warming potential (GWP-total) | GWP-b=Global warming potential - Biogenic (GWP-b) | GWP-f=Global warming potential - Fossil (GWP-f) | GWP-
luluc=Global warming potential - Land use and land use change (GWP-luluc) | EP-m=Eutrophication marine (EP-m) | EP-fw=Eutrophication, freshwater (EP-fw) | EP-T=Eutrophication,
terrestrial (EP-T) | ODP=Ozone depletion (ODP) | POCP=Photochemical ozone formation - human health (POCP) | ADP-f=Resource use, fossils (ADP-f) | ADP-mm=Resource use, minerals and
metals (ADP-mm) | WDP=Water use (WDP)
reinforcing stabilized three and seven-wire strands with and without dents with a nominal tensile strength of 1670÷1860 N /mm2 with a diameter of 6.5÷15.7 mm (PC-strand) . | ReTHiNK-62692 10 / 17
Environmental Product Declaration
5 Results
ADDITIONAL ENVIRONMENTAL IMPACT INDICATORS EN15084+A2
Abbreviation Unit A1 A2 A3 C1 C2 C3 C4 D
ETP-fw CTUe 3.49E+0 3.54E-1 3.23E+0 0.00E+0 9.53E-2 0.00E+0 4.77E-3 -4.54E+1
PM disease incidence 6.15E-3 1.68E-9 1.65E-4 0.00E+0 6.37E-10 0.00E+0 4.86E-11 -7.83E-8
HTP-c CTUh 1.23E-10 2.16E-11 1.03E-9 0.00E+0 3.09E-12 0.00E+0 1.10E-13 -1.75E-10
HTP-nc CTUh 1.12E-8 3.96E-10 1.28E-8 0.00E+0 1.04E-10 0.00E+0 3.39E-12 2.62E-7
IR kBq U235 eqv. 5.22E-2 1.85E-3 1.62E-2 0.00E+0 4.48E-4 0.00E+0 3.02E-5 2.31E-2
SQP Pt 1.64E+0 2.28E-1 8.33E-1 0.00E+0 9.27E-2 0.00E+0 1.54E-2 -2.09E+0
ETP-fw=Ecotoxicity, freshwater (ETP-fw) | PM=Particulate Matter (PM) | HTP-c=Human toxicity, cancer (HTP-c) | HTP-nc=Human toxicity, non-cancer (HTP-nc) | IR=Ionising radiation, human
health (IR) | SQP=Land use (SQP)
CLASSIFICATION OF DISCLAIMERS TO THE DECLARATION OF CORE AND ADDITIONAL ENVIRONMENTAL IMPACT INDICATORS
ILCD classification Indicator Disclaimer
Global warming potential (GWP) None
ILCD type / level 1 Depletion potential of the stratospheric ozone layer (ODP) None
Potential incidence of disease due to PM emissions (PM) None
AAcidification potential, Accumulated Exceedance (AP) None
Eutrophication potential, Fraction of nutrients reaching freshwater end compartment
None
(EP-freshwater)
Eutrophication potential, Fraction of nutrients reaching marine end compartment
ILCD type / level 2 None
(EP-marine)
Eutrophication potential, Accumulated Exceedance (EP-terrestrial) None
Formation potential of tropospheric ozone (POCP) None
Potential Human exposure efficiency relative to U235 (IRP) 1
Abiotic depletion potential for non-fossil resources (ADP-minerals&metals) 2
ILCD type / level 3
Abiotic depletion potential for fossil resources (ADP-fossil) 2
Water (user) deprivation potential, deprivation-weighted water consumption (WDP) 2
Potential Comparative Toxic Unit for ecosystems (ETP-fw) 2
Potential Comparative Toxic Unit for humans (HTP-c) 2
reinforcing stabilized three and seven-wire strands with and without dents with a nominal tensile strength of 1670÷1860 N /mm2 with a diameter of 6.5÷15.7 mm (PC-strand) . | ReTHiNK-62692 11 / 17
Environmental Product Declaration
5 Results
ILCD classification Indicator Disclaimer
Potential Comparative Toxic Unit for humans (HTP-nc) 2
Potential Soil quality index (SQP) 2
Disclaimer 1 – This impact category deals mainly with the eventual impact of low dose ionizing radiation on human health of the nuclear fuel cycle. It does not consider effects due to possible
nuclear accidents, occupational exposure nor due to radioactive waste disposal in underground facilities. Potential ionizing radiation from the soil, from radon and from some construction
materials is also not measured by this indicator.
Disclaimer 2 – The results of this environmental impact indicator shall be used with care as the uncertainties on these results are high or as there is limited experienced with the indicator.
5.2 INDICATORS DESCRIBING RESOURCE USE AND ENVIRONMENTAL INFORMATION BASED ON LIFE CYCLE INVENTORY (LCI)
PARAMETERS DESCRIBING RESOURCE USE
Abbreviation Unit A1 A2 A3 C1 C2 C3 C4 D
PERE MJ 4.94E-1 2.85E-2 1.63E-1 0.00E+0 1.34E-3 0.00E+0 5.95E-5 2.75E-1
PERM MJ 0.00E+0 0.00E+0 0.00E+0 0.00E+0 0.00E+0 0.00E+0 0.00E+0 0.00E+0
PERT MJ 4.94E-1 2.85E-2 1.63E-1 0.00E+0 1.34E-3 0.00E+0 5.95E-5 2.75E-1
PENRE MJ 2.60E+1 3.50E-1 2.44E+0 0.00E+0 1.13E-1 0.00E+0 7.82E-3 -9.81E+0
PENRM MJ 0.00E+0 0.00E+0 5.66E-2 0.00E+0 0.00E+0 0.00E+0 0.00E+0 0.00E+0
PENRT MJ 2.60E+1 3.50E-1 2.50E+0 0.00E+0 1.13E-1 0.00E+0 7.82E-3 -9.81E+0
SM Kg 1.67E-1 0.00E+0 5.16E-3 0.00E+0 0.00E+0 0.00E+0 0.00E+0 0.00E+0
RSF MJ 0.00E+0 0.00E+0 0.00E+0 0.00E+0 0.00E+0 0.00E+0 0.00E+0 0.00E+0
NRSF MJ 0.00E+0 0.00E+0 0.00E+0 0.00E+0 0.00E+0 0.00E+0 0.00E+0 0.00E+0
FW M3 1.19E-1 1.55E-4 1.84E-2 0.00E+0 1.30E-5 0.00E+0 7.86E-6 -4.89E-3
PERE=renewable primary energy ex. raw materials | PERM=renewable primary energy used as raw materials | PERT=renewable primary energy total | PENRE=non-renewable primary energy
ex. raw materials | PENRM=non-renewable primary energy used as raw materials | PENRT=non-renewable primary energy total | SM=use of secondary material | RSF=use of renewable
secondary fuels | NRSF=use of non-renewable secondary fuels | FW=use of net fresh water
reinforcing stabilized three and seven-wire strands with and without dents with a nominal tensile strength of 1670÷1860 N /mm2 with a diameter of 6.5÷15.7 mm (PC-strand) . | ReTHiNK-62692 12 / 17
Environmental Product Declaration
5 Results
OTHER ENVIRONMENTAL INFORMATION DESCRIBING WASTE CATEGORIES
Abbreviation Unit A1 A2 A3 C1 C2 C3 C4 D
HWD Kg 1.92E-9 6.42E-7 4.27E-6 0.00E+0 2.71E-7 0.00E+0 1.10E-8 -1.62E-4
NHWD Kg 2.36E-1 4.46E-3 1.01E-1 0.00E+0 6.78E-3 0.00E+0 5.00E-2 -1.32E-1
RWD Kg 6.56E-4 2.03E-6 3.01E-5 0.00E+0 7.02E-7 0.00E+0 4.83E-8 8.01E-6
HWD=hazardous waste disposed | NHWD=non hazardous waste disposed | RWD=radioactive waste disposed
ENVIRONMENTAL INFORMATION DESCRIBING OUTPUT FLOWS
Abbreviation Unit A1 A2 A3 C1 C2 C3 C4 D
CRU Kg 0.00E+0 0.00E+0 0.00E+0 0.00E+0 0.00E+0 0.00E+0 0.00E+0 0.00E+0
MFR Kg 4.52E-4 0.00E+0 2.55E-2 0.00E+0 0.00E+0 9.50E-1 0.00E+0 0.00E+0
MER Kg 0.00E+0 0.00E+0 0.00E+0 0.00E+0 0.00E+0 0.00E+0 0.00E+0 0.00E+0
EET MJ 0.00E+0 0.00E+0 1.40E-2 0.00E+0 0.00E+0 0.00E+0 0.00E+0 0.00E+0
EEE MJ 0.00E+0 0.00E+0 8.12E-3 0.00E+0 0.00E+0 0.00E+0 0.00E+0 0.00E+0
CRU=Components for re-use | MFR=Materials for recycling | MER=Materials for energy recovery | EET=Exported Energy Thermic | EEE=Exported Energy Electric
reinforcing stabilized three and seven-wire strands with and without dents with a nominal tensile strength of 1670÷1860 N /mm2 with a diameter of 6.5÷15.7 mm (PC-strand) . | ReTHiNK-62692 13 / 17
Environmental Product Declaration
5 Results
5.3 INFORMATION ON BIOGENIC CARBON CONTENT PER KILOGRAM
BIOGENIC CARBON CONTENT
The following Information describes the biogenic carbon content in (the main parts of) the
product at the factory gate per kilogram:
Biogenic carbon content Amount Unit
Biogenic carbon content in the product 0 kg C
Biogenic carbon content in accompanying packaging 0 kg C
reinforcing stabilized three and seven-wire strands with and without dents with a nominal tensile strength of 1670÷1860 N /mm2 with a diameter of 6.5÷15.7 mm (PC-strand) . | ReTHiNK-62692 14 / 17
Environmental Product Declaration
6 Interpretation of results
The graph illustrates the impact of various factors on the x-axis, representing different
indicator factors, while the legends denote the modules on the y-axis. With A1 having the
most impact and D having the most balancing impact. The main impact is from A1 as the
main input is Raw material and there are some small processes happening which has not
so much impact.
reinforcing stabilized three and seven-wire strands with and without dents with a nominal tensile strength of 1670÷1860 N /mm2 with a diameter of 6.5÷15.7 mm (PC-strand) . | ReTHiNK-62692 15 / 17
Environmental Product Declaration
7 References
ISO 14040
ISO 14040:2006-10, Environmental management - Life cycle assessment - Principles and
framework; EN ISO 14040:2006
ISO 14044
ISO 14044:2006-10, Environmental management - Life cycle assessment - Requirements
and guidelines; EN ISO 14040:2006
ISO 14025
ISO 14025:2011-10: Environmental labels and declarations — Type III environmental
declarations — Principles and procedures
EN 15804+A2
EN 15804+A2: 2019: Sustainability of construction works — Environmental Product
Declarations — Core rules for the product category of construction products
PCR A
PCR A – General Program Category Rules for Construction Products from the EPD
programme of Kiwa-Ecobility Experts; Version 2.1 (2022)
PCR B
Kiwa-Ecobility Experts, Berlin, 2020: PCR B – Product Category Rules for steel construction
products, Requirements on the Environmental Product Declarations for steel construction
products; Version 2020-03-13 (draft)
reinforcing stabilized three and seven-wire strands with and without dents with a nominal tensile strength of 1670÷1860 N /mm2 with a diameter of 6.5÷15.7 mm (PC-strand) . | ReTHiNK-62692 16 / 17
Environmental Product Declaration
8 Contact information
Publisher Operator Owner of declaration
Kiwa-Ecobility Experts Kiwa-Ecobility Experts PJSC "STALKANAT"
Voltastraße 5 Voltastraße 5 str. Vodoprovidna 16,
13355 Berlin, DE 13355 Berlin, DE 65007 Odesa, UA, UA
E-mail: E-mail: E-mail:
DE.Ecobility.Experts@kiwa.com DE.Ecobility.Experts@kiwa.com gremecheva_sb@stalkanat.com.ua
Website: Website: Website:
https://www.kiwa.com/de/en/themes/ecobility-experts/ecobility-https://www.kiwa.com/de/en/themes/ecobility-experts/ecobility-https://stalkanat.com.ua/
experts-epd-program/ experts-epd-program/
Kiwa-Ecobility Experts is
established member of the
reinforcing stabilized three and seven-wire strands with and without dents with a nominal tensile strength of 1670÷1860 N /mm2 with a diameter of 6.5÷15.7 mm (PC-strand) . | ReTHiNK-62692 17 / 17
