—
EPD
Environmental Product Declaration
REX640 Protection and Control Relay
Production site: Vaasa, Finland
DOCUMENT KIND IN COMPLIANCE WITH
Environmental Product Declaration ISO 14025 and EN 50693
PROGRAM OPERATOR PUBLISHER
The Norwegian EPD Foundation The Norwegian EPD Foundation
EPD-NORWAY REGISTRATION NUMBER AND DECLARATION NUMBER ISSUE DATE
NEPD-3951-2989-EN 2022-11-28
VALID TO STATUS SECURITY LEVEL
2027-11-28 Approved Public
OWNING ORGANIZATION DECLARATION NUMBER REV. LANG. PAGE
ABB Switzerland Ltd, Group Technology Management 2RCA057421 A en 1/24
© Copyright 2021 ABB. All rights reserved.
ver2-191222
ENVIRONMENTAL PRODUCT DECLARATION
EPD Owner ABB Swizerland Ltd, Group Technology Management
Organisation no CHE-101.538.426
Manufacturer name ABB Oy
and address Muottite 2 A, Vaasa, Finland
Seila Rodriguez-Vilches – seila.rodriguez-vilches@ch.abb.com
Sustainability Product Manager
Company contact
Jani Valtari – jani.valtari@fi.abb.com
R&D Manager
The Norwegian EPD Foundation
Post Box 5250 Majorstuen, 0303 Oslo, Norway
Program operator
phone: +47 23 08 80 00
email: post@epd-norge.no
REX640 Protection and Control Relay
FU: To protect a power system against faults such as short circuit
Declared product,
and overload, during a service life of 10 years and with a use rate of
functional unit (FU),
100 %.
and reference flow (RF)
RF: A single protection and control relay, including related
accessories and packaging.
The REX640 relay is used in utility, industrial, and transport and
infrastructure applications for protection, control, measurement, and
super-vision of power distribution systems. REX640 is based on an
application package concept, that offer a variety of ready-made
Product description application packages to choose from. The available application
packages provide feeder protection, power transformer protection,
machine protection, shunt capacitor protection, busbar protection,
automatic synchronization, Petersen coil control, Arc protection with
supervised sensors.
CPC code 4621 - Electricity distribution or control apparatus
Independent verification of the declaration and data, according to
ISO 14025:2010
☐INTERNAL ☒ EXTERNAL
Independent
Independent verifier approved by EPD-Norway: Elisabet Amat Guasch
verification
Signature:
Håkon Hauan, CEO EPD-Norge
Approved by
Signature:
Reference PCR and EPDItaly007 – PCR for Electronic and Electrical Products and
version number Systems, Rev. 2, 2020/10/21.
EN 50693:2019 - Product category rules for life cycle assessments of
Core PCR
electronic and electrical products and systems
10 years (this is a theoretical period selected for calculation purposes
Product RSL
only and it is not representative for the minimum, average, nor actual
description
service life of the product)
Markets of Global: Manufacturing and distribution
applicability Europe: Use and end-of-life
This EPD is based on the LCA study described in the LCA report
LCA study
2RCA057422
EPD type A specific product by a specific manufacturer
STATUS SECURITY LEVEL DOCUMENT ID. REV. LANG. PAGE
Approved Public 2RCA057421 A en 2/24
© Copyright 2021 ABB. All rights reserved.
ENVIRONMENTAL PRODUCT DECLARATION
EPD scope “Cradle to grave”
Year of reported
2021
primary data
LCA software SimaPro 9.3.0.3 (2022)
LCI database ecoinvent v3.8 (2021)
LCIA methodology EN 50693:2019
EPDs published within the same product category, though
originating from different programs, may not be comparable. Full
Comparability conformance with a PCR allows EPD comparability only when all
stages of a life cycle have been considered. However, variations and
deviations are possible.
The owner of the declaration shall be liable for the underlying
Liability information and evidence. EPD-Norway shall not be liable with
respect to manufacturer, life cycle assessment data and evidences.
STATUS SECURITY LEVEL DOCUMENT ID. REV. LANG. PAGE
Approved Public 2RCA057421 A en 3/24
© Copyright 2021 ABB. All rights reserved.
ENVIRONMENTAL PRODUCT DECLARATION
Contents
ABB Purpose & Embedding Sustainability ..................................................................................... 5
General Information ........................................................................................................................ 6
Constituent materials .................................................................................................................... 10
LCA background information ........................................................................................................ 11
Inventory analysis .......................................................................................................................... 15
Environmental indicators .............................................................................................................. 17
Additional environmental information ........................................................................................ 22
References...................................................................................................................................... 24
STATUS SECURITY LEVEL DOCUMENT ID. REV. LANG. PAGE
Approved Public 2RCA057421 A en 4/24
© Copyright 2021 ABB. All rights reserved.
ENVIRONMENTAL PRODUCT DECLARATION
ABB Purpose & Embedding Sustainability
ABB is a leading global technology company that energizes the transformation of society
and industry to achieve a more productive, sustainable future. By connecting software to
its electrification, robotics, automation and motion portfolio, ABB pushes the boundaries
of technology to drive performance to new levels. With a history of excellence stretching
back more than 130 years, ABB’s success is driven by about 110 thousand talented
employees in over 100 countries.
ABB's Electrification business offers a wide-ranging portfolio of products, digital
solutions and services, from substation to socket, enabling safe, smart and sustainable
electrification. Offerings encompass digital and connected innovations for low and
medium voltage, including EV infrastructure, solar inverters, modular substations,
distribution automation, power protection, wiring accessories, switchgear, enclosures,
cabling, sensing and control.
ABB is committed to continually promoting and embedding sustainability across its
operations and value chain, aspiring to become a role model for others to follow. With its
ABB Purpose, ABB is focusing on reducing harmful emissions, preserving natural
resources and championing ethical and humane behavior.
STATUS SECURITY LEVEL DOCUMENT ID. REV. LANG. PAGE
Approved Public 2RCA057421 A en 5/24
© Copyright 2021 ABB. All rights reserved.
ENVIRONMENTAL PRODUCT DECLARATION
General Information
REX640 is an all-in-one protection and control relay use in advanced power distribution
and generation applications with unmatched flexibility available during the complete life
cycle of the device. The relay has a modular design for both hardware and software, which
allows customization and modification flexibility, and adaptation to changing protection
requirements. REX640 relays are used in utility, industrial, and transport and
infrastructure applications for protection, control, measurement, and super-vision of
power distribution systems. REX640 is based on an application package concept, that
offer a variety of ready-made application packages to choose from. The available
application packages provide feeder protection, power transformer protection, machine
protection, shunt capacitor protection, busbar protection, automatic synchronization,
Petersen coil control, and Arc protection with supervised sensors throughout the relay life
cycle.
The products declared in this Environmental Product Declaration includes the
configurations of the REX640 protection and control relays.
General technical specifications for the REX640 are as follows:
Description Value
Width 304,0 mm
Height 264,8 mm
With compression type
242,2 mm
CT/VT connectors
With ring lug type
Depth 254,1 mm
CT/VT connectors
With grounding bar 274,0 mm
Weight (exc. packaging 6,9…9,3 kg
STATUS SECURITY LEVEL DOCUMENT ID. REV. LANG. PAGE
Approved Public 2RCA057421 A en 6/24
© Copyright 2021 ABB. All rights reserved.
ENVIRONMENTAL PRODUCT DECLARATION
Power Supply Power Supply Power Supply
Module 1001 Module 1002 Module 1003
Nominal auxiliary 24, 30, 48, 60 V DC 100, 110, 120, 220, 240 110, 125 V DC
voltage U V AC, 50 and 60 Hz
n
48, 60, 110, 125, 220,
250 V DC
Burden of auxiliary DC < 18,0 W AC < 20,0 W (nominal) DC < 17,0 W
voltage supply under (nominal) / / < 25,0 W (max.) (nominal) /
< 25,0 W (max.) < 25,0 W (max.)
quiescent (P ) /
q DC < 20,0 W (nominal)
operating condition
/ < 25,0 W (max.)
The REX640 protection and control relays are produced in Vaasa, Finland, and the relays
are sold globally.
The manufacturing site in Vaasa, Finland, uses 100 % renewable energy for the electricity,
more specifically, a 50/50 mix of wind and hydro. The plant is also certified according to
the following standards:
• ISO 9001:2015 – Quality management systems
• ISO 14001:2015 – Environmental management systems
• ISO 45001:2018 – Occupational health and safety management systems
Note, ABB only performs final assembling and testing of the relays. ABB does not
manufacture any parts or components themselves. Instead, this is outsourced and
purchased from various suppliers. Most of the parts are purchased as sub-assemblies or
ready modules.
STATUS SECURITY LEVEL DOCUMENT ID. REV. LANG. PAGE
Approved Public 2RCA057421 A en 7/24
© Copyright 2021 ABB. All rights reserved.
ENVIRONMENTAL PRODUCT DECLARATION
The relay has mandatory and optional slots. A mandatory slot always contains a module,
but an optional slot may be empty, depending on the configration ordered. The module
slots are shown in table 3.
Due to the modular nature of the product, there is a significant variation within the REX640 in
terms of environmental impacts. A representative relay is therefore selected as reference
product and declared in this EPD. The configuration of the reference product has all module
slots but one filled. The results of the study can be extrapolated for other relay
configurations according to EN 50693. The extrapolation rules are provided together with
the results.
STATUS SECURITY LEVEL DOCUMENT ID. REV. LANG. PAGE
Approved Public 2RCA057421 A en 8/24
© Copyright 2021 ABB. All rights reserved.
ENVIRONMENTAL PRODUCT DECLARATION
Slot Description Module
Base functionality REX640B10NN
A1 - -
A2 Communication module COM1002
B Binary input/output module BI01001
C Binary input/output module BI01001
D Binary input/output module BI01001
E Analogue input module 1 AIM1001
F Analogue input module 2 AIM1002
G Power supply module PSM1002
Product REX640
Average nominal power 16,5 W
Weight (excl. packaging) 9,16 kg
Ordering code REX640_11Z9
The ordering code is generated based on selected configuration in the ABB’s product
selection tool.
Packaging materials and manuals associated with these products are also included in the
study.
Description Material and weight
Manuals Printed paper, 43 g
Packaging box Cardboard,471 g
Box interior Moulded recycled fibre pulp, 384 g
Pallet (6 pcs / pallet) Wooden pallet, 1767 g
STATUS SECURITY LEVEL DOCUMENT ID. REV. LANG. PAGE
Approved Public 2RCA057421 A en 9/24
© Copyright 2021 ABB. All rights reserved.
ENVIRONMENTAL PRODUCT DECLARATION
Constituent materials
The reference product weighs ca 9,16 kg, including 7 slots of maximum 8 in terms of
hardware. Stickers and glue used in PSM base plate assembly have been excluded as they
are considered negligible to the overall environmental impacts. Due to the complex nature
of the electronics, these are presented as a separate category, which includes printed
wiring boards, electronic components, connectors, and cables. Electronics are typically
composed of various plastics, copper, and precious metals.
REX640 reference product (excl. packaging)
Materials Name CAS Number Weight [kg] %
Aluminium 7429-90-5 4,69 51
Steel, stainless steel 12597-68-1 0,26 3
Metals
Steel, low-alloyed 12597-69-2 0,14 2
Other metals 0,11 1
Electronics (PWBs, compo-
- 3,92 43
Others nents, connectors, cables)
Others - 0,04 0
9,16 100
REX640 reference product
Other metals1 %
Steel, low-alloyed2 % Others0 %
Steel, stainless steel3 %
Aluminum51 %
Electronics43 %
STATUS SECURITY LEVEL DOCUMENT ID. REV. LANG. PAGE
Approved Public 2RCA057421 A en 10/24
© Copyright 2021 ABB. All rights reserved.
ENVIRONMENTAL PRODUCT DECLARATION
LCA background information
Functional Unit and Reference Flow
The functional unit of this study is to protect a power system against faults such as short
circuit and overload, during a service life of 10 years and with a use rate of 100 %. The
reference flow is a single protection and control relay, including related accessories and
packaging.
Note, the reference service life (RSL) of 10 years is a theoretical period selected for
calculation purposes only – this is not representative for the minimum, average, nor actual
service life of the product.
System Boundaries
The life cycle analysis of the REX640, an EEPS (Electronic and Electrical Products and
Systems), is a “from cradle to grave” analysis and covers the following main life cycle
stages according to EN 50693: Manufacturing stage, including the relevant upstream pro-
cess (e.g. acquisition of raw material, preparation of semi-finished goods, etc.) and the
main manufacturing and processing steps; distribution stage; installation stage,
including the relevant steps for the preparation of the product for use; use stage,
including the re-quired maintenance steps within the RSL (reference service life)
associated to the reference product; end-of-life stage, including the necessary steps until
and for the final disposal or recovery of the product system.
STATUS SECURITY LEVEL DOCUMENT ID. REV. LANG. PAGE
Approved Public 2RCA057421 A en 11/24
© Copyright 2021 ABB. All rights reserved.
ENVIRONMENTAL PRODUCT DECLARATION
The following figure shows the stages of the product life cycle and the information stages
according to the PCR EPDItaly007 for the evaluation of electronic and electrical products
and systems.
M E M
A Manufacturing R Manufacturing A Distribution
O
E E
R Acquisition of raw C Assembly R Transport to distributor/
materials logistic center
T T
EoL treatment of
S S
Transport to generated waste Transport to place of use
P N
manufacturing site
U Packaging production W
Manufacturing of parts Installation
O
by ABB suppliers
D Installation
EoL treatment of generated
waste (packaging)
Use
Usage
End of Life
Collection and transport
EoL treatment
More specifically, the stages of the product life cycle and the information considered for
the evaluation of the REX640 are the following:
• The upstream manufacturing stage: This includes the acquisition of raw
materials as well as production and transportation of semi-finished parts,
components, and sub-assemblies from both direct and indirect suppliers to ABB.
Production losses are also included.
• The core manufacturing stage: This includes the final assembling and testing at
the local manufacturing site in Finland. It also includes the utility consumptions
and the waste generated at the sites as well as the production and use of
packaging materials.
• The distribution stage: This includes all activities related to the distribution and
transportation of the final product to the site of installation.
• The installation stage: This includes the end of life of the packaging materials.
• The use stage: This includes the power consumption throughout the reference
service life of the product.
• The end-of-life stage: This includes all activities related to waste treatment and
disposal of the product at the end of its service life.
STATUS SECURITY LEVEL DOCUMENT ID. REV. LANG. PAGE
Approved Public 2RCA057421 A en 12/24
© Copyright 2021 ABB. All rights reserved.
ENVIRONMENTAL PRODUCT DECLARATION
Temporal and geographical boundaries
The component suppliers are sourced all over the world: Africa, Asia and Europe. All
primary data collected from ABB are from 2021, which is a representative production year.
Secondary data are provided by ecoinvent v3.8.
Due to the unclear origin of each material, ecoinvent processes with a global
representativeness have been used. Thus, a conservative approach has been adopted.
Boundaries in the life cycle
In terms of boundaries, the PCR EPDitaly007 requires to refer to chapter 4.2.3.1 in the
standard EN 50693 for products that can be easily replaced or recovered. In accordance
with EN 50693:2019, capital goods such as machinery, tools, buildings, infrastructure,
packaging for internal transports, and administrative activities, which cannot be allocated
directly to the production of the reference product, are excluded.
Infrastructures, when present, such as processes deriving from the ecoinvent database
have not been excluded.
Data quality
Both primary and secondary data are used. The main sources for primary data are the bill
of materials as well as technical drawings and documents. Site specific foreground data
have been provided by ABB. For all processes for which primary are not available, generic
data originating from the ecoinvent v3.8 database, “allocation, cut-off by classification”,
are used. The ecoinvent database is available in SimaPro 9.3.0.3 which is the LCA software
used for the calculations.
Environmental impact indicators
The information obtained from the inventory analysis is aggregated according to the
effects related to the various environmental issues. In accordance with the PCR
EPDItaly007, the environmental impact indicators are determined by using the
characterization factors and impact assessment methods specified in EN
15804:2012+A2:2019.
Note, the PCR EPDItaly007 uses four different indicators for climate change (GWP-GHG):
GWP (total), which includes all greenhouse gases; GWP (fossil fuels); GWP (biogenic
carbon), which includes the emissions and absorption of biogenic carbon dioxide and
biogenic carbon stored in the product; GWP (land use).
STATUS SECURITY LEVEL DOCUMENT ID. REV. LANG. PAGE
Approved Public 2RCA057421 A en 13/24
© Copyright 2021 ABB. All rights reserved.
ENVIRONMENTAL PRODUCT DECLARATION
Allocation rules
The utility consumption and waste generation of the ABB’s production plant are allocated
to the production of one relay by using allocation rules. Because the plant is focused on
relay production, the total utility consumption and waste generation for 2021 are simply
divided by the total output of relays during the same year. Utility consumption and waste
generation deriving from offices and administrative activities are not excluded because it
is not possible to accurately allocate the inventory only for the production. Thus, a
conservative approach is adopted.
For the end-of-life allocation, the “polluter pays” principle is adopted according to what is
defined in the CEN/TR 16970 standard, as required by the PCR EPDItaly007. This means,
waste treatment processes are allocated to the product system that generates the waste
until the end-of-waste state is reached. The environmental burdens of recycling and
energy recovery processes are therefore allocated to the product system that generates
the waste, while the product system that uses the exported energy and recycled materials
receives it burden-free. However, the potential benefits and avoided loads from recovery
and recycling processes are not considered because it is not required by EPDItaly007.
Limitations and simplifications
The PCR EPDItaly007 does not provide any details about cut-off criteria; it refers to
chapter 4.2.3.3 in the standard EN 50693. According to EN 50693, the cut-off criteria can
be set to a maximum of 5 % of the overall environmental impacts given by the LCIA results.
In this study, stickers and glue used in PSM base plate assembly have been excluded as
they are considered negligible to the overall environmental impacts.
STATUS SECURITY LEVEL DOCUMENT ID. REV. LANG. PAGE
Approved Public 2RCA057421 A en 14/24
© Copyright 2021 ABB. All rights reserved.
ENVIRONMENTAL PRODUCT DECLARATION
Inventory analysis
In this study, both primary and secondary data are used. The main sources for primary
data are the bill of materials as well as technical drawings and documents. Site specific
foreground data have been provided by ABB. The ecoinvent v3.8 cut-off by classification
system processes are used to model the background system of the processes.
Due to the complex supply chain of the REX640, ecoinvent processes are selected with a
global representativeness.
Manufacturing stage
Aluminium and electronics are the most frequently used materials, followed by stainless
and low-alloyed steel.
To account for the production efforts of metal parts, “metal working, average”-processes
are most commonly used.
The printed wiring boards (PWB) are modelled on a component level. Thus, every single
component that is mounted on the PWBs is categorized and grouped into the most
corresponding component found in ecoinvent. Furthermore, due to the high impacts of
gold, primary data are used to model the specific amounts of gold used in each connector.
The transport distances of raw materials to the manufacturing site of the first known
supplier in the supply chain are assumed to be included in ecoinvent’s “market for”-
processes. Additional transports of semi-finished parts, components, and sub-
assemblies between indirect suppliers, direct suppliers, and ABB’s production plant are
added separately. Intercontinental transports are assumed to be by air. Thus, a
conservative approach is adopted.
The core manufacturing stage of the REX640 takes place in ABB manufacturing site in
Finland. The utility consumption and waste generation of the ABB’s production plant are
allocated to the production of one relay according to the provided allocation rules.
Packaging materials and manuals are also included in the analysis, in the core
manufacturing stage.
STATUS SECURITY LEVEL DOCUMENT ID. REV. LANG. PAGE
Approved Public 2RCA057421 A en 15/24
© Copyright 2021 ABB. All rights reserved.
ENVIRONMENTAL PRODUCT DECLARATION
Distribution
The relays are in general delivered directly to the customer, and the most common type of
transport is by road and air. ABB does not have any additional distribution centres. The
relays are neither repacked throughout the distribution stage.
A distribution scenario is developed based on primary data. A weighted average is
calculated for air, sea, and road transports based on delivery statistics from 2021.
Installation
The installation phase only implies manual activities, and no energy is consumed. Thus, in
the LCA, this phase only includes the end-of-life of the packaging materials and manuals
that are discarded after installation. Statistical data are adopted from Eurostat (2018) to
create a scenario which is representative for Europe. A transport distance of 100 km is
assumed because the actual location of disposal is unknown.
Use
The use phase considers the power consumption over the reference service life of 10 years
as defined in the functional unit. A use rate of 100 % is assumed because under normal
operational circumstances, the relay is always powered on in a stand-by mode. Variations
in power consumption from other modes are therefore considered negligible, including
power losses from input and output signals. Because this product is sold globally and is
not limited to any specific country, the latest energy mix for the European Union is
adopted as suggested by the standard EN 50693. The emission factor is derived from GWP
- total from the selected impact assessment method. For reference, the following table
shows the greenhouse gas emissions per kWh (EN 15804:2012+A2:2019 method, GWP
indicator):
Electricity mix Data source Amount Unit
European electricity mix:
Electricity, medium voltage {RER}| Ecoinvent v3.8 0,40 kg CO2-eq/kWh
market group for | Cut-off, S
End of life
The end-of-life stage is modelled according to the PCR EPDItaly007 and IEC/TR 62635. The
percentages for end-of-life treatments of the product are adopted from IEC/TR 62635
(Annex D, example 2), which is representative for Europe. The scenario is based on the
rates given for materials that go through a separation process and thus, a conservative
approach is adopted. A transport distance of 100 km is assumed because the distance to
the actual location of disposal is unknown.
STATUS SECURITY LEVEL DOCUMENT ID. REV. LANG. PAGE
Approved Public 2RCA057421 A en 16/24
© Copyright 2021 ABB. All rights reserved.
ENVIRONMENTAL PRODUCT DECLARATION
Environmental indicators
This chapter presents the environmental impact indicators for the selected reference
product of REX640, according to the PCR EPDItaly007. Extrapolation rules are thereafter
provided, based on a sensitivity analysis, which allows for estimating more precise
impacts of other relay configurations.
The indicators are divided into the contribution of the processes to the different modules
(upstream, core and downstream) and stages (manufacturing, distribution, installation,
use and end-of-life).
REX640 reference product
Product: REX640
Ordering code: REX640_11Z9
Hardware: 7 of 8 slots filled
Nominal power: 16,5 W (measured, average)
UPSTREAM CORE DOWNSTREAM
Impact category Unit Total
Manufacturing Distribution Installation Use End-of-life
GWP - total kg CO2 eq. 8,63E+02 2,35E+02 1,35E+00 4,13E+01 1,46E+00 5,77E+02 5,91E+00
GWP - fossil kg CO2 eq. 8,41E+02 2,33E+02 3,56E+00 4,13E+01 7,43E-02 5,58E+02 5,73E+00
GWP - biogenic kg CO2 eq. 1,97E+01 1,81E+00 -2,30E+00 1,46E-02 1,39E+00 1,86E+01 1,79E-01
GWP - luluc kg CO2 eq. 1,82E+00 4,25E-01 7,87E-02 3,00E-03 2,60E-05 1,31E+00 8,04E-04
ODP kg CFC-11 eq. 5,27E-05 1,52E-05 3,15E-07 9,40E-06 1,18E-08 2,76E-05 7,25E-08
AP mol H+ eq. 5,49E+00 2,24E+00 2,26E-02 2,15E-01 4,00E-04 3,00E+00 4,69E-03
EP - freshwater kg P eq. 8,42E-01 2,82E-01 1,53E-03 6,24E-04 1,00E-05 5,57E-01 2,52E-04
POCP kg NMVOC eq. 2,52E+00 1,04E+00 1,60E-02 2,23E-01 4,54E-04 1,24E+00 4,07E-03
ADP – minerals
kg Sb eq. 8,62E-02 8,48E-02 4,55E-05 1,64E-05 2,20E-07 1,32E-03 8,29E-06
and metals
MJ, net calorific
ADP – fossil 1,54E+04 2,87E+03 4,91E+01 5,80E+02 8,60E-01 1,19E+04 8,98E+00
value
WDP m3 eq. 2,18E+02 8,58E+01 2,36E+00 4,99E-01 -6,37E-03 1,29E+02 1,73E-01
GWP-fossil: Global Warming Potential fossil; GWP-biogenic: Global Warming Potential biogenic; GWP-luluc: Global Warming
Potential land use and land use change; ODP: Depletion potential of the stratospheric ozone layer; AP: Acidification potential;
EP-freshwater: Eutrophication potential-freshwater compartment; POCP: Formation potential of tropospheric ozone; ADP-
minerals & metals: Abiotic Depletion for non-fossil resources potential; ADP-fossil: Abiotic Depletion for fossil resources potential,
WDP: Water deprivation potential.
STATUS SECURITY LEVEL DOCUMENT ID. REV. LANG. PAGE
Approved Public 2RCA057421 A en 17/24
© Copyright 2021 ABB. All rights reserved.
ENVIRONMENTAL PRODUCT DECLARATION
Resource UPSTREAM CORE DOWNSTREAM
use Unit Total
parameters Manufacturing Distribution Installation Use End-of-life
MJ, low cal.
PENRE 1,54E+04 2,81E+03 4,90E+01 5,80E+02 8,60E-01 1,19E+04 8,98E+00
value
MJ, low cal.
PERE 2,54E+03 3,23E+02 9,09E+01 2,14E+00 1,54E-02 2,12E+03 7,14E-01
value
MJ, low cal.
PENRM 5,66E+01 5,66E+01 0,00E+00 0 0 0 0
value
MJ, low cal.
PERM 4,32E+01 0 4,32E+01 0 0 0 0
value
MJ, low cal.
PENRT 1,54E+04 2,87E+03 4,90E+01 5,80E+02 8,60E-01 1,19E+04 8,98E+00
value
MJ, low cal.
PERT 2,58E+03 3,23E+02 1,34E+02 2,14E+00 1,54E-02 2,12E+03 7,14E-01
value
FW m3 1,33E+01 2,96E+00 1,54E-01 1,91E-02 -5,89E-05 1,01E+01 6,42E-03
MS kg 3,73E+00 3,37E+00 3,60E-01 0 0 0 0
RSF MJ 0 0 0 0 0 0 0
NRSF MJ 0 0 0 0 0 0 0
PENRE: Use of non-renewable primary energy excluding non-renewable primary energy resources used as raw material; PERE:
Use of renewable primary energy excluding renewable primary energy resources used as raw material; PENRM: Use of non-
renewable primary energy resources used as raw material; PERM: Use of renewable primary energy resources used as raw
material; PENRT: Total use of non-renewable primary energy resources (primary energy and primary energy resources used as
raw materials); PERT: Total use of renewable primary energy resources (primary energy and primary energy resources used as
raw materials); FW: Net use of fresh water; MS: Use of secondary materials; RFS: Use of renewable secondary fuels, NRSF: Use
of non-renewable secondary fuels.
Waste UPSTREAM CORE DOWNSTREAM
production Unit Total
indicators Manufacturing Distribution Installation Use End-of-life
HWD kg 3,89E-02 3,30E-02 1,19E-04 1,54E-03 2,15E-06 4,23E-03 1,71E-05
NHWD kg 7,64E+01 3,32E+01 9,58E-01 1,66E+00 1,39E-01 3,95E+01 9,32E-01
RWD kg 1,00E-01 8,13E-03 1,91E-04 4,11E-03 5,03E-06 8,80E-02 4,00E-05
MER kg 3,09E+00 0 5,45E-01 0 8,79E-01 0 1,67E+00
MFR kg 9,92E+00 1,23E+00 1,58E+00 0 1,72E+00 0 5,40E+00
CRU kg 0 0 0 0 0 0 0
ETE MJ 1,92E+01 0 1,63E+00 0 3,09E+00 0 1,45E+01
EEE MJ 9,82E+00 0 7,99E-01 0 1,54E+00 00 7,49E+00
HWD: hazardous waste disposed; NHWD: non-hazardous waste disposed; RWD: radioactive waste disposed; MER: materials
for energy recovery; MFR: material for recycling; CRU: components for reuse; ETE: exported thermal energy; EEE: exported
electricity energy.
STATUS SECURITY LEVEL DOCUMENT ID. REV. LANG. PAGE
Approved Public 2RCA057421 A en 18/24
© Copyright 2021 ABB. All rights reserved.
ENVIRONMENTAL PRODUCT DECLARATION
Extrapolation rules
Due to the large variations in environmental impacts present within the REX640,
extrapolation rules are established according to EN 50693. The rules are based on a
sensitivity analysis and the changes in percentages are presented in tables in the
following pages, in relation to the reference product. This allows for estimating more
precise impacts of other relay configurations. The following rules are established:
1. The upstream manufacturing stage, distribution stage, and end-of-life stage can be
extrapolated based on the number of hardware modules.
• Range of variation: 0–4 empty slots
• Reference product: 1 empty slot
• Formula for 2-4 empty slots: 𝑉𝑎𝑙𝑢𝑒 ∗(1−𝑐ℎ𝑎𝑛𝑔𝑒%∗(𝑛 −1))
refproduct emptyslots
• Formula for 0 empty slots: 𝑉𝑎𝑙𝑢𝑒 ∗(1+ 𝑐ℎ𝑎𝑛𝑔𝑒%∗0,31)
refproduct
2. The use stage can be extrapolated based on the actual, measured nominal power
consumption.
• Formula: 𝑉𝑎𝑙𝑢𝑒 ∗(1−𝑐ℎ𝑎𝑛𝑔𝑒%∗(16,5−P ))
𝑟𝑒𝑓𝑝𝑟𝑜𝑑𝑢𝑐𝑡 nominal
• Range of variation: 12–20 W
Example 1: A REX640 relay that have 3 hardware module slots empty, and a measured
nominal power consumption at 15 W.
• GWP-total in upstream stage = 235,0 kg CO -eq * (1 – 9 % * (3 – 1) = 192,5 kg CO -eq
2 2
• GWP-total in use stage = 577,5 kg CO -eq * (1 – 16,5% * (16,5–15)) = 525,0 kg CO -eq
2 2
Example 2: REX640 relay that have 0 hardware module slots empty, and a measured
nominal power consumption at 18 W.
• GWP-fossil in distribution = 41,3 kg CO -eq * (1 + 6 % * 0,31) = 42,0 kg CO -eq
2 2
• GWP-fossil in use stage = 557,5 kg CO -eq * (1 – 6,1 ,5% * (16,5-18)) = 608,2 kg CO -eq
2 2
An REX640 extrapolation tool with changeable parameters is provided in:
https://search.abb.com/library/Download.aspx?DocumentID=2RCA057534&LanguageC
ode=en&DocumentPartId=&Action=Launch
STATUS SECURITY LEVEL DOCUMENT ID. REV. LANG. PAGE
Approved Public 2RCA057421 A en 19/24
© Copyright 2021 ABB. All rights reserved.
ENVIRONMENTAL PRODUCT DECLARATION
Change per hardware module Change per Watt
Impact
category Upstream Core
Distribution Installation Use End-of-life Use
manufacturing manufacturing
GWP - total 9,0 % - 6,0 % - - 15,3 % 6,1 %
GWP - fossil 9,1 % - 6,0 % - - 15,7 % 6,1 %
GWP -
3,3 % - 5,9 % - - 0,6 % 6,1 %
biogenic
GWP - luluc 7,9 % - 6,2 % - - 4,9 % 6,1 %
ODP 9,2 % - 6,0 % - - 6,8 % 6,1 %
AP 10,9 % - 6,1 % - - 8,0 % 6,1 %
EP -
10,4 % - 6,0 % - - 5,7 % 6,1 %
freshwater
POCP 9,7 % - 6,1 % - - 9,7 % 6,1 %
ADP –
minerals and 11,1 % - 6,0 % - - 2,2 % 6,1 %
metals
ADP – fossil 9,6 % - 6,0 % - - 6,0 % 6,1 %
WDP 9,8 % - 6,0 % - - 10,7 % 6,1 %
GWP-fossil: Global Warming Potential fossil; GWP-biogenic: Global Warming Potential biogenic; GWP-luluc: Global Warming
Potential land use and land use change; ODP: Depletion potential of the stratospheric ozone layer; AP: Acidification potential;
EP-freshwater: Eutrophication potential-freshwater compartment; POCP: Formation potential of tropospheric ozone; ADP-
minerals & metals: Abiotic Depletion for non-fossil resources potential; ADP-fossil: Abiotic Depletion for fossil resources
potential, WDP: Water deprivation potential.
Change per hardware module Change per Watt
Resource use
parameters Upstream Core
Distribution Installation Use End-of-life Use
manufacturing manufacturing
PENRE 9,4 % - 6,0 % - - 6,0 % 6,1 %
PERE 9,3 % - 6,0 % - - 4,4 % 6,1 %
PENRM 19,2 % - - - - - -
PERM - - - - - - -
PENRT 9,6 % - 6,0 % - - 6,0 % 6,1 %
PERT 9,3 % - 6,0 % - - 4,4 % 6,1 %
FW 9,0 % - 6,0 % - - 9,7 % 6,1 %
MS 0,4 % - - - - - -
RSF - - - - - - -
NRSF - - - - - - -
PENRE: Use of non-renewable primary energy excluding non-renewable primary energy resources used as raw material; PERE:
Use of renewable primary energy excluding renewable primary energy resources used as raw material; PENRM: Use of non-
renewable primary energy resources used as raw material; PERM: Use of renewable primary energy resources used as raw
material; PENRT: Total use of non-renewable primary energy resources (primary energy and primary energy resources used as
raw materials); PERT: Total use of renewable primary energy resources (primary energy and primary energy resources used as
raw materials); FW: Net use of fresh water; MS: Use of secondary materials; RFS: Use of renewable secondary fuels, NRSF: Use
of non-renewable secondary fuels.
STATUS SECURITY LEVEL DOCUMENT ID. REV. LANG. PAGE
Approved Public 2RCA057421 A en 20/24
© Copyright 2021 ABB. All rights reserved.
ENVIRONMENTAL PRODUCT DECLARATION
Waste Change per hardware module Change per Watt
production
Upstream Core
indicators Distribution Installation Use End-of-life Use
manufacturing manufacturing
HWD 8,4 % - 5,9 % - - 8,2 % 6,1 %
NHWD 8,9 % - 6,0 % - - 4,4 % 6,1 %
RWD 9,3 % - 6,0 % - - 5,4 % 6,1 %
MER - - - - - 17,1 % -
MFR 1,0 % - - - - 2,6 % -
CRU - - - - - - -
ETE - - - - - 17,1 % -
EEE - - - - - 17,1 % -
HWD: hazardous waste disposed; NHWD: non-hazardous waste disposed; RWD: radioactive waste disposed; MER: materials for
energy recovery; MFR: material for recycling; CRU: components for reuse; ETE: exported thermal energy; EEE: exported
electricity energy.
STATUS SECURITY LEVEL DOCUMENT ID. REV. LANG. PAGE
Approved Public 2RCA057421 A en 21/24
© Copyright 2021 ABB. All rights reserved.
ENVIRONMENTAL PRODUCT DECLARATION
Additional environmental information
Recyclability potential
The recyclability potential of the reference product is calculated by dividing “MFR: material
for recycling” with the total weight of the relay. This is based on the end-of-life scenario
adopted from IEC/TR 62635 (Annex D, example 2) which is representative for Europe. The
scenario is based on the rates given for materials that go through a separation process,
and the production losses in the recycling processes have also been considered; thus, a
conservative approach is adopted. Recyclability potentials for other relay configurations
are also provided, which is based on a sensitivity analysis and extrapolation procedures.
Product Recyclability potential
REX640, full relay (extrapolated) 58,5 %
REX640, 1 slot empty (reference product) 58,9 %
REX640, 2 slots empty (extrapolated) 62,8 %
REX640, 3 slots empty (extrapolated) 66,7 %
REX640, 4 slots empty (extrapolated) 70,6 %
REACH and RoHS compliance of REX640
As part of ABB’s values, and in alignment with the Supplier Code of Conduct, we seek to
work with companies who contribute to a sustainable development and are ethically,
socially, environmentally, and economically responsible.
ABB is responsible for ensuring that our products comply with legal requirements. There
are also other sets of environmental requirements not necessarily originating from
legislation, but which are of great importance as ABB customers are demanding
compliance with them.
ABB Distribution Solutions has contacted suppliers of REX640 to collect component and
material information. This information includes, but is not limited to:
• Full Material Disclosure
• RoHS compliance certificate
• REACH compliance certificate
• Component lifecycle status
Thus, the purpose is to avoid chemicals, materials and substances that
• may represent hazards to the environment, or
• the health of workers, customers, consumers and other stakeholders, or
• could negatively influence end-of-life properties.
STATUS SECURITY LEVEL DOCUMENT ID. REV. LANG. PAGE
Approved Public 2RCA057421 A en 22/24
© Copyright 2021 ABB. All rights reserved.
ENVIRONMENTAL PRODUCT DECLARATION
Additional Norwegian requirements
Greenhouse gas emissions from the use of electricity in the
manufacturing phase
Production mix from green energy purchasing certificate medium voltage (production of
transmission lines, in addition to direct emissions and losses in grid) applied electricity
for the manufacturing process.
Electricity mix Data source Amount Unit
ABB FI – custom:
Ecoinvent v3.8 0,0259 kg CO2-eq/kWh
50 % wind + 50 % hydro
Dangerous substances
The product contains no substances given by the REACH Candidate list.
Indoor environment
The product meets the requirements for low emissions.
Carbon footprint
Carbon footprint has not been worked out for the product.
STATUS SECURITY LEVEL DOCUMENT ID. REV. LANG. PAGE
Approved Public 2RCA057421 A en 23/24
© Copyright 2021 ABB. All rights reserved.
ENVIRONMENTAL PRODUCT DECLARATION
References
• Kurki, M. (2022). REX640 Life Cycle Assessment Report 2RCA057422
• EN 50693:2019 – Product category rules for life cycle assessments of electronic and
electrical products and systems
• EN 15804:2012+A2:2019 – Sustainability of constructions - Environmental product
declarations (September 2019)
• PCR EPDItaly007 – Electronic and electrical products and systems (rev.2), October
2020
• IEC/TR 62635 – Guidelines for end-of-life information provided by manufacturers and
recyclers and for recyclability rate calculation of electrical and electronic equipment -
Edition 1.0 2012-10
• ISO 14025:2010 – Environmental labels and declarations - Type III environmental
declarations - Principles and procedures
• ISO 14040:2006 - Environmental management - Life cycle assessment - Principles
and framework
• ISO 14044:2006 - Environmental management - Life cycle assessment -
Requirements and guidelines
• Ecoinvent, 2021. Swiss Centre for Life Cycle Assessment, v3.8 (www.ecoinvent.ch)
• PRé Consultants, 2022. Software SimaPro version 9.3.0.3. (www.pre.nl)
• Eurostat (2018) – treatment of waste by waste category, hazardousness and waste
management operations.
(http://appsso.eurostat.ec.europa.eu/nui/show.do?lang=en&dataset=env_wastrt)
• EN 16258:2012 – Methodology for calculation and declaration of energy consumption
and GHG emissions of transport services (freight and passengers)
• EPDItaly Regulations rev. 5.2 (16th February 2022)
• General Programme Instructions for The Norwegian EPD Foundation/EPD-Norway
(www.epd-norge.no) version 5:2019
Program Operator and publisher Ph. +47 23 08 80 00
The Norwegian EPD Foundation
Post Box 5250 Majorstuen, email post@epd-norge.no
0303 Oslo, Norway web www.epd-norge.no
Owner of the declaration
ABB Swizerland Ltd, Group
Technology Management
Brown Boveri Straße 6, 5400
web www.abb.com
Baden, Switzerland
Author Ph. +358 50 334 1214
Martina Kurki
ABB Oy email martina.kurki@fi.abb.com
Muottitie 2 A, Vaasa, Finland web www.abb.com
STATUS SECURITY LEVEL DOCUMENT ID. REV. LANG. PAGE
Approved Public 2RCA057421 A en 24/24
© Copyright 2021 ABB. All rights reserved.
