ENVIRONMENTAL PRODUCT DECLARATION
as per ISO 14025 and EN 15804+A2
Owner of the Declaration RHEINZINK GmbH & Co. KG
Publisher Institut Bauen und Umwelt e.V. (IBU)
Programme holder Institut Bauen und Umwelt e.V. (IBU)
Declaration number EPD-RHE-20230366-IBA2-EN
Issue date 02/01/2024
Valid to 01/01/2029
RHEINZINK-prePATINA® blue-grey and graphite-grey
RHEINZINK GmbH & Co. KG
www.ibu-epd.com | https://epd-online.com
1. General Information
RHEINZINK GmbH & Co. KG RHEINZINK-prePATINA® blue-grey and graphite-
grey
Programme holder Owner of the declaration
IBU – Institut Bauen und Umwelt e.V. RHEINZINK GmbH & Co. KG
Hegelplatz 1 Bahnhofstraße 90
10117 Berlin 45711 Datteln
Germany Germany
Declaration number Declared product / declared unit
EPD-RHE-20230366-IBA2-EN 1 kg of RHEINZINK®-prePATINA
This declaration is based on the product category rules: Scope:
Building metals, 04/07/2023 The Life Cycle Assessment (LCA) was carried out according to DIN ISO
(PCR checked and approved by the SVR) 14044. Specific data from the company RHEINZINK in Datteln, Germany,
and from the database Sphera LCA FE were used. The LCA was carried
out for the manufacturing phase of the products, taking into account all
Issue date background data such as raw material production and transports ('cradle to
gate'). The use phase of the titanium zinc sheets is divided into several
02/01/2024
application areas: roofing applications, roof drainage and facade
claddings. The treatment for the titanium zinc sheets was modelled in re-
melting furnaces for the end-of-life phase. The thereby resulting credit of
Valid to
extracted zinc is counted as replacement for primary zinc.
01/01/2029 The owner of the declaration shall be liable for the underlying information
and evidence; the IBU shall not be liable with respect to manufacturer
information, life cycle assessment data and evidences.
The EPD was created according to the specifications of EN 15804+A2. In
the following, the standard will be simplified as EN 15804.
Verification
The standard EN 15804 serves as the core PCR
Independent verification of the declaration and data according to ISO
14025:2011
Dipl.-Ing. Hans Peters internally X externally
(Chairman of Institut Bauen und Umwelt e.V.)
Florian Pronold Ms Jane Anderson,
(Managing Director Institut Bauen und Umwelt e.V.) (Independent verifier)
1 Environmental Product Declaration - RHEINZINK GmbH & Co. KG - RHEINZINK-prePATINA® blue-grey and graphite-grey
2. Product
Name Value Unit
2.1 Product description/Product definition
Coefficient of thermal expansion 22 10-6K-1
The basis of RHEINZINK®-prePATINA is electrolytic special
high-grade zinc in accordance with EN 1179. Added to this are Tensile strength /EN 10002-1/ ≥150 N/mm2
small amounts of titanium and copper based on EN 988. In Modulus of elasticity ≥80000 N/mm2
addition to other factors, the alloy composition is not only
Melting point 420 °C
important for the technological material properties of
Thermal conductivity 109 W/(mK)
RHEINZINK®, but also for the colour of its patina. The
RHEINZINK®-prePATINA blue-grey and graphite-grey surface Electrical conductivity at 20°C 17x10^6 Ω-1m-1
is the result of a chemical pickling process. This preweathering Density 7200 kg/m3
process anticipates the colour of the typical natural patina,
which will develop during the period of use.
2.4 Delivery status
For the placing on the market in the EU and European Free
The material RHEINZINK® is delivered in thicknesses from 0.5
Trade Association (EFTA) (with the exception of Switzerland)
– 1.5 mm. The maximum width of strips and sheets is 1.000
the Regulation (EU) No. 305/2011 applies. The products need a
mm. The standard sheets are delivered in 1x2 m and 1x3 m,
Declaration of Performance taking into consideration EN 14782
coils are delivered with a maximum weight of 1 t. Finished
or EN 14783 respectively and the CE-marking.
products are delivered to customer specifications.
For the application and use the respective national provisions
Application rules
apply.
EN 988, Zinc and zinc alloys - Specification for rolled flat
2.2 Application products for building
• Titanium zinc sheets, strips and profiles for roofing and facade
EN 506, Roofing products from metal sheet- specification for
cladding according to EN 14782 -Self-supporting metal sheet
self-supporting products of copper and zinc sheet
for roofing, external cladding and internal lining according to EN
14783 - Fully supported metal sheet and strip for roofing,
EN 612, Eaves gutters with bead stiffened fronts and rainwater
external cladding and internal lining. The products are CE-
pipes with seamed joints made of metal sheet
marked based on these standards.
2.5 Base materials/Ancillary materials
• Roof drainage systems (roof gutters, pipes and accessories)
-Components of RHEINZINK-alloy
according to EN 612 - Eaves gutters with bead stiffened fronts
and rainwater pipes with seamed joints made of metal sheet. • Special-High-Grade zinc 99.995% (Z1 according to DIN
EN 1179)
2.3 Technical Data • Copper: 0.1 - 0.18% (blugrey)
The following table gives conversion data from product surface • Copper: 0.9 - 1.0% (graphite grey)
mass per unit area for the relevant product systems in roofing, • Titanium: 0.07 - 0.12%
facade cladding and roof drainage. • Aluminium: ≤ 0.015%
-Auxiliary substances
RHEINZINK® is an alloy of zinc with small amounts of copper
and titanium. No compound of the alloy >0.1% is listed in the
'Candidate List of Substances of Very High Concern for
Authorisation' (SVHC) dated 01/2018. The product does not
contain any substances with carcinogenic, mutagenic,
reprotoxic (CMR) properties > 0.1%. RHEINZINK products do
not contain biocide properties as defined by the (EU) Ordinance
on Biocide Products No. 528/2012). Lubricant emulsion (rolling
process): 0.08 kg/t zinc
2.6 Manufacture
Structure of the manufacturing process:
The manufacturing process comprises seven steps:
Pre-alloy:
To improve the quality, and for energy-saving reasons, a pre-
alloy is produced at 760 °C in an induction crucible (melting of
SHG zinc, copper, titanium and aluminium). The pre-alloy
blocks produced contain the titanium and copper portions of the
subsequently rolled alloy.
Performance data of the product in accordance with the
respective declaration of performance with respect to its
Melting:
essential characteristics according to EN 14782 and EN 14783
The pre-alloy blocks and SHG zinc are melted together in large
respectively.
melting furnaces (induction furnaces) at 500 – 550 °C and
Constructional data mixed by induction currents.
2 Environmental Product Declaration - RHEINZINK GmbH & Co. KG - RHEINZINK-prePATINA® blue-grey and graphite-grey
Casting:
The final alloy is cooled down below melting point by a closed 2.10 Condition of use
water circuit in the casting machine, resulting in a solid cast RHEINZINK® is UV-resistant and does not rot. It is resistant to
string. a rust film, non-flammable and resistant to radiating heat and
against most of the chemical substances used in building
Rolling: construction. Effects on the durability of RHEINZINK® products
There is a cooling distance between the casting machine and with regard to snow, rain and hail are not known. The effects of
the roller racks. The rolling is done by 5 roller pairs, so-called snow and rain may be neglected.
roller racks. With adequate pressures the material thickness is
reduced by up to 50% at each of these roller racks. This material has a repellent effect to electro-smog
Simultaneously, the material is cooled and greased (electromagnetic radiation in excess of 98%).
using a special emulsion.
RHEINZINK® develops a superficial protective coating, the so-
Coiling: called patina, which darkens only slightly over the years and
Subsequently, the finished rolled RHEINZINK® is wound up which is responsible for the high resistance of zinc against
into coils of 20 tonnes. They are still at a temperature of 100- corrosion. In the chemical process that forms this patina, zinc
150 °C and are stored for further cooling. oxide develops in contact with the oxygen in the air. Next, due
to the influence of water (precipitation), zinc hydroxide
Preweathering: develops, which will be transformed into a tight, strongly
The surface appearance is achieved by a pickling process. The adhering and non-water-soluble coating of basic zinc carbonate
material is degreased, rinsed, then pickled in an acidic pickling (patina) in reaction with the carbon dioxide in the air. Therefore
bath, rinsed again, and then provided with a thin antifingerprint RHEINZINK® does not require any maintenance and cleaning
coating (1-2 µm thickness). The process is identical for during the period of use.
bluegrey and graphite grey, the difference in colour results from
the different copper concentration. 2.11 Environment and health during use
Environmental aspects:
Stretching and cutting: The transfer of zinc ions via rainwater is constantly reduced due
The tensions developed inside the RHEINZINK® bands during to the development of the natural protecting coat of zinc
rolling are 'stretched-out' by a stretching-bending-straightening carbonate (Patina). The further transfer of zinc ions depends
process. mainly on air contamination with 'acid' pollutants, particularly
The trimming scrap produced during the manufacturing of the with SO . As a result of the reduction of SO concentration in
2 2
material is 100% remelted at RHEINZINK GmbH & Co. KG and
the air to 20% of the former values during the last 30 years, the
processed into new products.
zinc concentration of precipitation has subsequently been
reduced by the same amount in the rainwater. The runoff rate is
Quality control:
2,0 - 3,0 g/m²/year. The total zinc concentration has been lower
Control by the manufacturer. Quality management according to
than the prescriptive limits for drinking water. In aquatic
ISO 9001.
systems only a small part of the total zinc concentration is
available for an organism - this amount is called bioavailable. It
2.7 Environment and health during manufacturing
is related to the physical-chemical conditions of the receiving
Environmental management according to ISO 14001. Energy
water body. The bioavailability is for example influenced by the
management according to ISO 50001. These management
amount of zinc which is organically or inorganically bound,
systems ascertain that the legal requirements concerning
linked to particles or competes with other ions.
worker health and environmental protection are fulfilled. Best
Available Technology is used throughout the plant.
Health aspects:
2.8 Product processing/Installation There will be no effects on health if the RHEINZINK® products
are used according to their designated function. Zinc, like iron,
Basic principles:
During transportation and storage, RHEINZINK® must be kept belongs to the essential metals. Zinc is not accumulated in the
body. The recommended daily intake of zinc according to the
dry and ventilated to avoid the formation of zinc hydroxide. For
Deutsche Gesellschaft für Ernährung (DGE - German Society
the same reason, when laying RHEINZINK® on wet surfaces or
for Nutrition) is 15 mg.
in the rain it should be ensured that the base material does not
have hygroscopic properties.
Lit.:
R. H. J. Korenromp et al, "Diffusive Emissions of zinc due to
The thermic stretching of the material has to be taken into
atmospheric corrosion of zinc and coated (galvanised)
consideration when handling/installing the product. Due to the
materials", TNO-MEP R99/441 (1999)
typical brittleness of zinc under cold conditions, the temperature
of the product during installation should be 10 °C. In other 2.12 Reference service life
cases, adequate mechanical equipment should be used, e.g.
Service lifetime according to BBSR (the Federal Office for
hot air blasts.
Building and Regional Planning): > 50 years, theoretical lifetime
according to available literature > 100 years. The standard ISO
2.9 Packaging
15686 has not been considered.
The packaging materials in use, paper/cardboard, polyethylene
(PE foils), polypropylene (PP foils) and steel, are recyclable 2.13 Extraordinary effects
(non-reusable wooden pallets, reusable wooden and metal
Fire
pallets). If gathered separately, return in Germany is organized
The RHEINZINK® products comply with DIN 4102, Part 1 and
by INTERSEROH which collects the packaging material at
to DIN EN 13501-1 the Requirements of Building Material Class
given sites with exchangeable containers upon request and
A1 'non-combustible'.
complies with legal regulations. The reusable wooden and steel
pallets are taken back and reimbursed by RHEINZINK GmbH &
Co. KG and the wholesale trade (refund system).
3 Environmental Product Declaration - RHEINZINK GmbH & Co. KG - RHEINZINK-prePATINA® blue-grey and graphite-grey
Fire protection
2.14 Re-use phase
Name Value End of life
Building material class EN 13501, DIN 4102 A1 When renovating or disassembling a building end of life,
Burning droplets EN 13501 D0 RHEINZINK® products can easily be collected. The cuttings
Smoke gas development EN 13501 - occurring at building sites as well as used zinc from renovation
sites are gathered and may be sent directly or via scrap-
gathering organizations to secondary melting plants - several
Smoke production/smoke concentration:
exist in Germany. The energy necessary for recycling titanium
When heated above 650 °C vaporization as zinc oxide (ZnO)
zinc sheets is only 5% of the primary energy content of zinc.
occurs.
The demand for zinc scrap, resulting from zinc recycling's low
energy requirement, is also mirrored by the fact that generally
Toxicity of the fumes:
about 70% of the value of the zinc content is reimbursed.
The ZnO smoke may cause zinc fever (diarrhoea, fever, dry
According to the newest information, the total recycling rate is
throat) when inhaled over a longer period of time, this
up to 96%.
disappears completely 1 to 2 days after inhalation.
2.15 Disposal
A small amount of zinc is weathered away, and another small
Water amount might be lost during collection and erroneously
Zinc is not classified as hazardous for the aquatic environment, disposed. All in all, this amounts to less than 4%. The European
WFD -European water framework directive. Waste Code according to Commission decision 2000/532/EC2
for zinc is 17 04 04.
Mechanical destruction
None 2.16 Further information
Additional information: www.rheinzink.de
3. LCA: Calculation rules
of energy usage and mass.
3.1 Declared Unit
3.5 Background data
Declared unit
The background data has been taken from the latest available
The declared unit is 1kg RHEINZINK®-prePATINA.
Sphera LCA FE (GaBi) database CUP 2023.1. Special High-
Name Value Unit Grade Zinc of the International Zinc Association (IZA) has been
Declared unit 1 kg used.
Gross density 7200 kg/m3
3.6 Data quality
The process data and the used background data are
3.2 System boundary
consistent.
Type of the EPD: cradle to gate - with options. In this study, the
Regarding foreground data, this study is based on high-quality
product stage information modules A1, A2, and A3 are
primary data, collected by RHEINZINK. Data were delivered in
considered. These modules include the production of raw
form of Excel tables and were checked for plausibility.
material extraction and processing (A1), processing of
Therefore, the data quality can be described as good.
secondary material input (A1), transport of the raw materials to
the manufacturer (A2), manufacturing of the product (A3) and 3.7 Period under review
packaging materials (A3). Modul A5 covers the waste treatment Modelling is based on production data from 2022.
of packaging materials (incineration of paper, plastic and Background data refer from 2019 to 2024.
wood). The special high-grade zinc allows an input of
secondary material of 1.5% zinc scrap. The post-consumer 3.8 Geographic Representativeness
scrap is used to saturate this input and is discounted from the Land or region, in which the declared product system is
material flow of module D. The transport to module C4 is manufactured, used or handled at the end of the product´s
considered under module C2. There is no activity declared for lifespan: Germany
C1.
Module C4 considers the non-recovered scrap due to losses
3.9 Allocation
and sorting efficiency as described in 2.15. There is no activity
in C3. In this study, allocation was avoided wherever possible.
The EoL of the product (Module D) is also included. The However, the following allocations had to be done:
treatment (remelting process of zinc scrap) and credits for • Credits from recycling from the end of life of the product
avoided primary production are grouped into module D. (Module D)
3.3 Estimates and assumptions 3.10 Comparability
No assumptions and estimations were necessary for the LCA. Basically, a comparison or an evaluation of EPD data is only
possible if all the data sets to be compared were created
3.4 Cut-off criteria
according to EN 15804 and the building context, respectively
All inputs and outputs to a (unit) process are included in the
the product-specific characteristics of performance, are taken
calculation, for which data were
into account. The background data has been taken from the
available. The applied cut–off criteria is 1% of renewable and
latest available Sphera LCA FE (GaBi) database CUP 2023.1.
non-renewable primary energy usage and 1% of the total mass
Special High-Grade Zinc of the International Zinc Association
input of that unit process in case of insufficient input data or
(IZA) has been used.
data gaps for a unit process. The total of neglected input flows
per module, e.g. per module A, B, C or D is a maximum of 5%
4 Environmental Product Declaration - RHEINZINK GmbH & Co. KG - RHEINZINK-prePATINA® blue-grey and graphite-grey
4. LCA: Scenarios and additional technical information
utilization (C2)
Characteristic product properties of biogenic carbon Modul C3:
The total mass of biogenic carbon-containing materials, in this The material reaches the end of waste state after transport to
case, cardboard and wooden pallets, is less than 5% of the the re-melters so there is no activity.
total mass of the product and accompanying packaging.
Information on describing the biogenic carbon content at Modul C4:
factory gate 500 km transport by 40 to truck, EURO 6, 61% average
utilization (C2)
Name ValueUnit
kg
Biogenic carbon content in product -
C
Modul A4, B1, B2, B3, B4, B5, reference service life, B6, B7
Biogenic carbon content in accompanying kg and C1 are not considered and declared in this study.
0.02
packaging C
The credits given in Module D result from the 100% recyclability
Note: 1 kg of biogenic carbon is equivalent to 44/12 kg of CO .
2
of each zinc-product. After the scrap collection (a collection rate
of 95% was assumed), zinc scrap is sent to a re-melting
process, where the scrap is converted to secondary zinc. The
Scenario Modul A5
credit for the zinc gained through re-melting is calculated with
Cardboard: 0,006 kg/kg product sent to incineration
the dataset of the primary production.
Wooden pallets: 0,03 kg/kg product sent to incineration
(exported Energy credited in Modul D) End of life (C4)
Plastic film: 0,001kg/kg product sent to incineration (exported Name Value Unit
Energy credited in Modul D)
Landfilling 5 %
Steel wrapping band Mass 3,41E-5 kg sent to recycling
(material recycling credited in Modul D) Reuse, recovery and/or recycling potentials (D), relevant
Modul C1: scenario information
No activity reported
Name Value Unit
Modul C2:
Recycling 95 %
500 km transport by 40 to truck, EURO 6, 61% average
5 Environmental Product Declaration - RHEINZINK GmbH & Co. KG - RHEINZINK-prePATINA® blue-grey and graphite-grey
5. LCA: Results
DESCRIPTION OF THE SYSTEM BOUNDARY (X = INCLUDED IN LCA; MND = MODULE OR INDICATOR NOT DECLARED; MNR
= MODULE NOT RELEVANT)
Benefits and
Construction loads beyond
Product stage Use stage End of life stage
process stage the system
boundaries
la ire ta m w a Ry lp p u s tro p s n a rT g n iru tc a fu n a M e h t m o rf tro p s n a rTe tis e h t o t e ta g y lb m e s s A e s U e c n a n e tn ia M ria p e R tn e m e c a lp e R tn e m h s ib ru fe R y g re n e la n o ita re p Oe s u re ta w la n o ita re p Oe s u n o itc u rts n o c -e Dn o itilo m e d tro p s n a rT g n is s e c o rp e ts a W la s o p s iD -e s u e R-y re v o c e R-g n ilc y c e Rla itn e to p
A1 A2 A3 A4 A5 B1 B2 B3 B4 B5 B6 B7 C1 C2 C3 C4 D
X X X MND X MND MND MNR MNR MNR MND MND X X X X X
RESULTS OF THE LCA - ENVIRONMENTAL IMPACT according to EN 15804+A2: 1 kg RHEINZINK®-prePATINA
Parameter Unit A1-A3 A5 C1 C2 C3 C4 D
GWP-total kg CO 2 eq 3.13E+00 5.69E-02 0 7.44E-03 0 2.39E-03 -2.13E+00
GWP-fossil kg CO 2 eq 3.17E+00 3.83E-03 0 7.42E-03 0 2.42E-03 -2.12E+00
GWP-biogenic kg CO 2 eq -4.75E-02 5.31E-02 0 -2.7E-05 0 -2.77E-05 -3.9E-03
GWP-luluc kg CO 2 eq 2.9E-03 3.2E-07 0 4.41E-05 0 2.38E-06 -2.26E-03
ODP kg CFC11 eq 4.86E-13 1.08E-14 0 1.82E-15 0 3.86E-15 1.5E-12
AP mol H+ eq 1.55E-02 1.26E-05 0 8.69E-06 0 7.5E-06 -1.19E-02
EP-freshwater kg P eq 7.17E-06 3.01E-09 0 1.74E-08 0 2.12E-09 -4.69E-06
EP-marine kg N eq 4.09E-03 3.43E-06 0 3.08E-06 0 1.88E-06 -2.97E-03
EP-terrestrial mol N eq 4.36E-02 5.54E-05 0 3.69E-05 0 2.07E-05 -3.15E-02
kg NMVOC
POCP 1.08E-02 9.04E-06 0 7.61E-06 0 5.9E-06 -7.77E-03
eq
ADPE kg Sb eq 1.54E-03 8.15E-11 0 5.32E-10 0 6.4E-11 -1.38E-03
ADPF MJ 4.27E+01 1.6E-02 0 1E-01 0 3.49E-02 -2.81E+01
m3 world eq
WDP 9.88E-01 6.38E-03 0 3.87E-05 0 -3.18E-05 -8.59E-01
deprived
GWP = Global warming potential; ODP = Depletion potential of the stratospheric ozone layer; AP = Acidification potential of land and water; EP =
Eutrophication potential; POCP = Formation potential of tropospheric ozone photochemical oxidants; ADPE = Abiotic depletion potential for non-fossil
resources; ADPF = Abiotic depletion potential for fossil resources; WDP = Water (user) deprivation potential)
RESULTS OF THE LCA - INDICATORS TO DESCRIBE RESOURCE USE according to EN 15804+A2: 1 kg RHEINZINK®-
prePATINA
Parameter Unit A1-A3 A5 C1 C2 C3 C4 D
PERE MJ 1.8E+01 6.37E-01 0 6.73E-03 0 3.14E-03 -1.46E+01
PERM MJ 6.32E-01 -6.32E-01 0 0 0 0 0
PERT MJ 1.86E+01 5.29E-03 0 6.73E-03 0 3.14E-03 -1.46E+01
PENRE MJ 4.29E+01 6.54E-02 0 1.01E-01 0 3.5E-02 -2.84E+01
PENRM MJ 4.94E-02 -4.94E-02 0 0 0 0 0
PENRT MJ 4.3E+01 1.6E-02 0 1.01E-01 0 3.5E-02 -2.84E+01
SM kg 1.11E-04 0 0 0 0 0 9E-01
RSF MJ 0 0 0 0 0 0 0
NRSF MJ 0 0 0 0 0 0 0
FW m3 4.4E-02 1.5E-04 0 5.99E-06 0 3.94E-07 -3.74E-02
PERE = Use of renewable primary energy excluding renewable primary energy resources used as raw materials; PERM = Use of renewable primary
energy resources used as raw materials; PERT = Total use of renewable primary energy resources; PENRE = Use of non-renewable primary energy
excluding non-renewable primary energy resources used as raw materials; PENRM = Use of non-renewable primary energy resources used as raw
materials; PENRT = Total use of non-renewable primary energy resources; SM = Use of secondary material; RSF = Use of renewable secondary fuels;
NRSF = Use of non-renewable secondary fuels; FW = Use of net fresh water
RESULTS OF THE LCA – WASTE CATEGORIES AND OUTPUT FLOWS according to EN 15804+A2:
1 kg RHEINZINK®-prePATINA
Parameter Unit A1-A3 A5 C1 C2 C3 C4 D
HWD kg 6.08E-04 7.69E-14 0 1.69E-13 0 2.89E-12 -1.46E+01
NHWD kg 1.66E+00 9.57E-04 0 1.5E-05 0 5.01E-02 0
RWD kg 5.18E-03 5.46E-07 0 1.32E-07 0 4.06E-07 -1.46E+01
CRU kg 0 0 0 0 0 0 -2.83E+01
MFR kg 0 1.53E-04 0 0 9.5E-01 0 0
MER kg 2.6E-02 3.62E-02 0 0 0 0 -2.83E+01
EEE MJ 5.42E-02 7.76E-02 0 0 0 0 9E-01
EET MJ 1.01E-01 1.46E-01 0 0 0 0 0
6 Environmental Product Declaration - RHEINZINK GmbH & Co. KG - RHEINZINK-prePATINA® blue-grey and graphite-grey
HWD = Hazardous waste disposed; NHWD = Non-hazardous waste disposed; RWD = Radioactive waste disposed; CRU = Components for re-use;
MFR = Materials for recycling; MER = Materials for energy recovery; EEE = Exported electrical energy; EET = Exported thermal energy
RESULTS OF THE LCA – additional impact categories according to EN 15804+A2-optional:
1 kg RHEINZINK®-prePATINA
Parameter Unit A1-A3 A5 C1 C2 C3 C4 D
Disease
PM ND ND ND ND ND ND ND
incidence
IR kBq U235 eq ND ND ND ND ND ND ND
ETP-fw CTUe ND ND ND ND ND ND ND
HTP-c CTUh ND ND ND ND ND ND ND
HTP-nc CTUh ND ND ND ND ND ND ND
SQP SQP ND ND ND ND ND ND ND
PM = Potential incidence of disease due to PM emissions; IR = Potential Human exposure efficiency relative to U235; ETP-fw = Potential comparative
Toxic Unit for ecosystems; HTP-c = Potential comparative Toxic Unit for humans (cancerogenic); HTP-nc = Potential comparative Toxic Unit for humans
(not cancerogenic); SQP = Potential soil quality index
Disclaimer 1 – for the indicator “Potential Human exposure efficiency relative to U235”. This impact category deals mainly with the
eventual impact of low-dose ionizing radiation on human health of the nuclear fuel cycle. It does not consider effects due to possible
nuclear accidents, occupational exposure or radioactive waste disposal in underground facilities. Potential ionizing radiation from the
soil, radon and from some construction materials is also not measured by this indicator.
Disclaimer 2 – for the indicators “abiotic depletion potential for non-fossil resources”, “abiotic depletion potential for fossil resources”,
“water (user) deprivation potential, deprivation-weighted water consumption”, “potential comparative toxic unit for ecosystems”,
“potential comparative toxic unit for humans – cancerogenic”, “Potential comparative toxic unit for humans - not cancerogenic”,
“potential soil quality index”. The results of this environmental impact indicator shall be used with care as the uncertainties on these
results are high as there is limited experience with the indicator.
6. LCA: Interpretation
The figures below show the relative contributions of the The high credits given in module D are the results of the 100%
production stages (Module A1-A3), transport to waste treatment recyclability of the zinc products. At the EoL of the zinc products
(Module C2), waste treatment (Module C4) and the benefits a collection rate of 95% was assumed. The 5% remaining is
and loads beyond the product system boundary (Module D). forwarded to the waste treatment (module C4). Overall, C2 and
C4 have a minimized contribution. Compared to RHEINZINK®-
The production of the high-grade zinc is the dominating CLASSIC bright-rolled, some of the differences in the results
contributor (87%-100%) to the indicators of the impact can be associated with the pickling process needed to produce
assessment as main raw material, followed by the generation of the RHEINZINK®-prePATINA, including the treatment of the
electricity. In the case of the ODP, module D is positive due to zinc sludge.
re-melting process where the emission of dichloro-1-
fluoroethane (R 141b) increases the impact, precursors of
Polyvinylidene fluorine (PVDF) used in the production of PV
modules.
7 Environmental Product Declaration - RHEINZINK GmbH & Co. KG - RHEINZINK-prePATINA® blue-grey and graphite-grey
7. Requisite evidence
Runoff rates roofs) suggest that small test racks may overestimate the run-
In a report of TNO-MEP-R99/441, a literature study was off rate.
undertaken to determine the runoff rates of zinc in Europe.
The decrease in the corrosion rates runs parallel to the
The following conclusions were taken in this report: decrease in the ambient concentrations of SO which is
2,
generally accepted as the dominant air pollution factor
Corrosion rates refer to the loss of metallic zinc, initially determining the corrosion of zinc.
accumulating as ionic zinc in the
patina layer. Run-off rates refer to the 'wash-off' of ionic zinc Corrosion rates decrease with time due to the increasing
from the patina layer, the difference being the amount of zinc protection of the patina layer. Therefore, long-term (20 years)
remaining in the patina layer. Run-off rates will in general be average corrosion rates will be substantially lower (60% of
lower than corrosion rates or at maximum equal to the initial value) than those during the first years of fresh not
corrosion rates. patinated materials. After a period of about 10 years, the run-off
rate will be approximately 2/3 of the corrosion rate.
Available data for corrosion and run-off rate result from
exposure of standard test panels Run-off rates can be calculated to be 3 g/m²/a in areas with
mounted on standard test racks. Only little data are available higher SO concentrations and 2 g/m²/a in areas with lower
2
from testing (on) real objects under the variety of typical
concentrations.
microclimate conditions to which they are exposed. Recent
experimental data with very large test racks (simulating zinc
8. References
EN 612:2005
EN 612:2005, Eaves gutters with bead stiffened fronts and ISO 15686:2011
rainwater pipes with seamed joints made of metal sheet ISO 15686:2011, Buildings and constructed assets - Service life
planning
EN 988:1996
EN 988:1996, Zinc and zinc alloys ISO 50001:2018
ISO 50001:2018, Energy Management System - Requirements
EN 1179:2003 with guidance for use
EN 1179:2003, Zinc and zinc alloys- Primary zinc
DIN 4102:1998 Bundesinstitut für Bau-, Stadt- und Raumforschung
DIN 4102:1998, Fire behaviour of building materials and (BBSR): 'Nutzungsdauer von Bauteilen für
building components Lebenszyklusanalysen nach BNB' (BNB: Bewertungssystem
Nachhaltiges Bauen) (2011)
ISO 9001:2015
ISO 9001:2015, Quality management systems – Requirements (EU) 305/2011
REGULATION (EU) No 305/2011 OF THE EUROPEAN
EN 10002:2001 PARLIAMENT AND OF THE COUNCIL
EN 10002:2001, Metallic materials - Tensile testing of 9 March 2011, laying down harmonised conditions for the
marketing of construction products and repealing Council
DIN EN 13501:2019 Directive 89/106/EEC
DIN EN 13501:2019, Fire classification of construction products
and building elements (EU) 528/2012
REGULATION (EU) No 528/2012 OF THE EUROPEAN
ISO 14001:2015 PARLIAMENT AND OF THE COUNCIL
ISO 14001:2015, Environmental management systems - of 22 May 2012, concerning the making available on the market
Requirements with guidance for use and use of biocidal products
DIN EN ISO 14040:2021 European waste catalogue
DIN EN ISO 14040:2021, Environmental management - Life Commission decision 2000/532/EC2
cycle assessment
Sphera LCA FE
DIN ISO 14044:2018 Sphera LCA FE Software and Databases for Life Cycle
DIN ISO 14044:2018, Environmental management - Life cycle Engineering. Sphera Solutions GmbH, Hauptstraße 111-113,
assessment – Requirements and guidelines 70771 Leinfelden-Echterdingen, Germany / Deutschland
EN 14782:2006 Hullmann, Heinz (Ed.):
EN 14782:2006, Self-supporting metal sheet for roofing, Natürlich oxidierende Metalloberflächen; Umweltauswirkungen
external cladding and internal lining beim Einsatz von Kupfer und Zink in Gebäudehüllen (Naturally
oxidising metal surfaces; environmental effects when using
EN 14783:2013 copper and zinc for buildings) ; 2003, Stuttgart, Fraunhofer ISB-
EN 14783:2013, Fully supported metal sheet and strip for Verlag, ISBN: 3-8167-6218-2.
roofing, external cladding and internal lining. The products are
CE-marked based on these standards
8 Environmental Product Declaration - RHEINZINK GmbH & Co. KG - RHEINZINK-prePATINA® blue-grey and graphite-grey
IZA 2012 for Construction Products from the range of Environmental
Special high grade zinc dataset, Developed by thinkstep AG, Product Declarations of Institut Bauen und Umwelt (IBU), Part
Owned by International Zinc Association, 2012, http://gabi- B: Requirements on the EPD for Building metals. July 2023
documentation-2018.gabi-software.com/xml- www.ibu-epd.de
data/processes/83e3e42c-0cc9-459b-960b-5fbda1280237.xml
TNO-MEP-R99/441
PCR 2022, Part A TNO-MEP-R99/441, Diffusive emissions of zinc due to
Institut Bauen und Umwelt e.V., Berlin: Product Category Rules atmospheric corrosion of zinc and zinc coated (galvanized)
for Building-Related Products and Services from the range of materials, 11-1999
Environmental Product Declarations of Institut Bauen und
Umwelt (IBU), Part A: Calculation Rules for the Life Cycle Directive 2000/60/EG (Water Framework Directive, WFD)
Assessment and Requirements on the Project Report. August DIRECTIVE 2000/60/EG OF THE EUROPEAN PARLIAMENT
2022 AND OF THE COUNCIL
www.ibu-epd.de of 23 October 2000, establishing a framework for Community
action in the field of water policy
PCR 2023, Part B
Institut Bauen und Umwelt e.V., Berlin: Product Category Rules
9 Environmental Product Declaration - RHEINZINK GmbH & Co. KG - RHEINZINK-prePATINA® blue-grey and graphite-grey
Publisher
Institut Bauen und Umwelt e.V. +49 (0)30 3087748- 0
Hegelplatz 1 info@ibu-epd.com
10117 Berlin www.ibu-epd.com
Germany
Programme holder
Institut Bauen und Umwelt e.V. +49 (0)30 3087748- 0
Hegelplatz 1 info@ibu-epd.com
10117 Berlin www.ibu-epd.com
Germany
Author of the Life Cycle Assessment
Sphera Solutions GmbH +49 (0)711 341817-0
Hauptstraße 111- 113 info@sphera.com
70771 Leinfelden-Echterdingen www.sphera.com
Germany
Owner of the Declaration
RHEINZINK GmbH & Co. KG +49 2363 605-0
Bahnhofstraße 90 info@rheinzink.de
45711 Datteln www.rheinzink.de
Germany
10 Environmental Product Declaration - RHEINZINK GmbH & Co. KG - RHEINZINK-prePATINA® blue-grey and graphite-grey
