ENVIRONMENTAL PRODUCT DECLARATION
as per ISO 14025 and EN 15804+A1
Owner of the Declaration ROCKWOOL International A/S
Publisher Institut Bauen und Umwelt e.V. (IBU)
Programme holder Institut Bauen und Umwelt e.V. (IBU)
Declaration number EPD-RWI-20190158-CCC2-EN
Issue date 01.11.2019
Valid to 30.04.2025
Rockpanel Durable & FS-Xtra
ROCKWOOL International A.S.
www.ibu-epd.com | https://epd-online.com
General Information
ROCKWOOL International A.S. Rockpanel Durable & FS-Xtra
Programme holder Owner of the declaration
IBU – Institut Bauen und Umwelt e.V. ROCKWOOL International A/S
Hegelplatz 1 Hovedgaden 584
10117 Berlin 2640 Hedehusene
Germany Denmark
Declaration number Declared product / declared unit
EPD-RWI-20190158-CCC2-EN 1 m2 of Rockpanel (Durable or A2 (FS-Xtra)) cladding panel
This declaration is based on the product category rules: Scope:
Mineral insulating materials, 01.08.2021 This declaration refers to Durable and A2 (FS-Xtra) cladding panels,
(PCR checked and approved by the SVR) produced by Rockpanel, a member of ROCKWOOL Group. The declared
reference product in this EPD is 1m2 Rockpanel Durable Cladding
Panel for facade cladding, roof detailing, soffits and fascias.
Issue date The Rockpanel products presented in this declaration are produced in
Roermond (Netherlands). For the Rockpanel A2 (FS-Xtra) cladding panel,
01.11.2019
the environmental impacts and indicators are determined by applying the
appropriate scaling factor (please refer to section "Technical Data" for
guidance).
Valid to
The production data correspond to the full year 2017.
30.04.2025 The owner of the declaration shall be liable for the underlying information
and evidence; the IBU shall not be liable with respect to manufacturer
information, life cycle assessment data and evidences.
The EPD was created according to the specifications of EN 15804+A1. In
the following, the standard will be simplified as EN 15804.
Verification
The standard EN 15804 serves as the core PCR
Independent verification of the declaration and data according to ISO
14025:2011
Dipl.-Ing. Hans Peters
internally X externally
(Chairman of Institut Bauen und Umwelt e.V.)
Florian Pronold Dr. Frank Werner,
(Managing Director Institut Bauen und Umwelt e.V.) (Independent verifier)
1 Environmental Product Declaration - ROCKWOOL International A.S. - Rockpanel Durable & FS-Xtra
Product
according to European Assessment Document (EAD) no. EAD
Product description/Product definition 090001-00-0404 for Prefabricated compressed mineral wool
Rockpanel stone wool facade panels are prefabricated boards with organic or inorganic finish and with specified
compressed mineral wool products with thermosetting binders. fastening system, edition May 2014.
The technical specifications for the products described in the
They are traditionally made from volcanic rock (typically basalt EPD are given by the range below based on the reference
or dolomite), and of recycled material and finished with a cured standards. For the product specific characteristics please refer
(waterborne) coating. to the manufacturer's specifications, available online in
http://www.rockpanel.com/.
The unfaced and coated synthetic resin-bonded stone wool
Constructional data
products described in this declaration are produced in the form
In the table below the first value refers to Durable and the
of panels in densities of 1050 kg/m3 for the Durable and 1250
second refers to A2 (FS-Xtra):
kg/m3 for the A2 (FS-Xtra) panel.
Name Value Unit
For the placing of the product on the market in the European
Union/European Free Trade Association (EU/EFTA) (with the Thermal conductivity acc.
0.37 - 0.55 W/(mK)
exception of Switzerland) the Regulation (EU) No. 305/2011 to EN 10456
(CPR) applies. The product needs a declaration of performance mm x
Maximum board size 3050x1250
taking into consideration: mm
• ETA-07/0141 from 15/12/2014 for Rockpanel Durable 8 Density (nominal) acc. to
1050/1250 kg/m³
mm finish Colours/Rockclad and Rockpanel Durable 8 EN 323
mm finish ProtectPlus, Mass (nominal) 8.40/11.25 kg/m²
• ETA-08/0343 of 16/09/2014 Rockpanel Durable 6 mm
Characteristic bending length and width f₀₅
finish Colours / Rockclad,
strength acc. to EN 3120; greater than or equal to N/mm²
• ETA-13/0340 of 18/01/2018 Rockpanel A2 (FS-Xtra) 9
EN 1058 27/25,5 (N/mm2)
mm finish Colours/Rocklad, Rockpanel A2 (FS-Xtra)
Modulus of elasticity acc.
9mm finish Structures and Rockpanel A2 (FS-Xtra) 9mm 4015/4740 N/mm²
to EN 310
finish ProtectPlus,
Vapour transmission Sd at
• ETA-13/0648 of 02/11/2015 Rockpanel Natural Durable
23°C and 65% RH acc. to 1.8 - 3.5 m
8 mm and 10 mm / Rockpanel Natural Xtreme 8 mm
ISO 12572:2016
and 10 mm.
• ETA-18/0883 of 2018/12/03 Dimensional Stability acc. mm/(m
11x10⁻³/10x10⁻³
Rockpanel Premium A2. to EN 438-2 °K)
For the application and use the respective national provisions
Performance data of the product in accordance with the
apply.
declaration of performance with respect to its essential
characteristics according to the following:
Application
The Rockpanel Durable and A2 (FS-Xtra), which are contained • ETA-07/0141 from 15/12/2014 for Rockpanel Durable 8
in this EPD, are cladding panels for facade applications. The mm finish Colours/Rockclad and Rockpanel Durable 8
Rockpanel Durable is offered with a density of 1050 kg/m3 and mm finish ProtectPlus,
thicknesses of 6, 8 and 10 mm. A2 (FS-Xtra) has a density of • ETA-08/0343 of 16/09/2014 Rockpanel Durable 6 mm
1250 kg/m3 and thicknesses of 9 mm and 11 mm. finish Colours / Rockclad,
• ETA-13/0340 of 18/01/2018 Rockpanel A2 (FS-Xtra) 9
Product-specific environmental impacts are compiled by
mm finish Colours/Rockclad, Rockpanel A2(FS-Xtra)
applying the relevant scaling factor (listed in the Scaling Factor
9mm finish structures and Rockpanel A2 (FS-Xtra) 9
table) in the Product Specific Scaling formula.
mm finish ProtectPlus,
• ETA-13/0648 of 02/11/2015 Rockpanel Natural Durable
8 mm and 10 mm / Rockpanel Natural Xtreme 8 mm
and 10 mm,
• ETA-18/0883 of 2018/12/03 Rockpanel Premium A2.
Base materials/Ancillary materials
The average composition used for this EPD is the following
(based on the average factory consumption figures for
Rockpanel production):
• non-scarce natural stone [18%]
• cement [10%]
Product Specific Scaling Formula: • slags and other secondary materials or waste materials
Environmental Impact per m2 = Environmental Impact [56%]
reference
• mineral oil and bonding agent [0,4%]
* scaling factor Please note that the scaling factors give
product • binder [12%]
a good indication of the impacts but they are not an exact • coating [3,6%]
measure as such. Packaging represents 5% of the final product delivered to the
customer. The raw materials are non-scarce stones, secondary
Technical Data
materials and briquettes, which are made of rock mineral wool
For the products where the above declared properties apply,
waste, secondary materials and by-products from other
the performance data are in accordance with the declaration of
industries such as slags, alumina and wool waste and cement.
performance with respect to its essential characteristics
2 Environmental Product Declaration - ROCKWOOL International A.S. - Rockpanel Durable & FS-Xtra
The binder is a phenol formaldehyde resin which is polymerized products produced in Europe fulfil the Note Q requirements.
into solid resin during the production of the final stone wool This is certified by the independent certification body EUCEB
product. The coating is a waterborne acrylic coating and an (European Certification Board for mineral wool products). More
additional (optional) PU coating. information on EUCEB can be found under www.euceb.org.
This product/article/at least one partial article contains
substances listed in the candidate list (ECHA PR/19/12) (date: Reference service life
16.07.2019) exceeding 0.1 percentage by mass: no. Assumed intended working life of the Rockpanel boards is 60
Mineral wool fibres produced by ROCKWOOL are classified as years, provided that they are subject to appropriate use and
non-hazardous under REACH (Regulation (EC) No 1272/2008 maintenance. This is in line with the results of an independent
of the European Parliament and of the council of 16 December accelerated durability test, done by Bouw Technologie and
2008 on classification, labelling and packaging of substances available from Rockpanel Group upon request. It is expected
and mixtures). ROCKWOOL are registered with REACH under that under normal use conditions the actual service life will be
the following definition: 'Man-made vitreous (silicate) fibres with considerably longer without major degradation affecting the
random orientation with alkaline oxide and alkali earth oxide essential requirements. Indications given as to the working life
(Na2O+K2O+CaO+MgO+BaO) content greater than 18% by of the boards cannot be interpreted as a guarantee given by
weight and fulfilling one of the Note Q conditions'. ROCKWOOL ROCKWOOL B.V. / Rockpanel.
LCA: Calculation rules
The transport in A4 is modelled based on the amount of panels
Declared Unit that fit in the truck.The values are based on annual average
The specific product referred to in the declared unit is 1 m2 of delivery data. In A5 the default installation is assumed to be
Rockpanel Durable cladding panel. The reference product has manual, therefore no energy consumption or ancillary
a thickness of 8 mm and a density of 1050 kg/m3. equipment is needed. The product waste from installation is
assumed to be 5% and according to the modularity principle of
Declared unit
EN 15804, its impacts are fully allocated to A5.
Name Value Unit
The A5 stage, according to EN 15804 includes also waste
Declared unit 1 m2 processing up to the end-of-waste state or disposal of final
Gross density 1050 kg/m3 residues during the construction process stage and impacts
and aspects related to product losses during installation.
Grammage 8.4 kg/m2
Finally, the A5 module includes also the corresponding end-of-
Surface 1 m2 life considerations for packaging. The default assumption here
Layer thickness 0.008 m for installation waste is 100% landfill.
Weight 8,4 kg
Building Use
conversion factor 8.4 -
The use-stage B1-B7, related to the building fabric
includes:
System boundary
• B1 use or application of the installed product- not part of
EPD type: Cradle to gate with options, modules C1–C4, and
this EPD;
module D. The modules considered in the life cycle
• B2 maintenance;
assessment as per system boundaries are described as
• B3 repair;
follows:
• B4 replacement;
Production
• B5 refurbishment;
The product stage A1-A3 includes:
• B6 – Operational energy use:
Provision of preliminary products and energy and relevant
• B7 – Operational water use:
upstream processes;
Rockpanel Stone wool cladding panel is installed permanently
• Transporting the raw materials and preliminary materials
in the structure and does not require maintenance, repair,
to ROCKWOOL production facilities;
replacement or refurbishment under normal use conditions.
• Production process in the ROCKWOOL production
Similarly, Rockpanel has no operational energy or water use.
facilities including energy inputs and emissions;
Rockpanel Durable waterborne coating used on the Rockpanel
• Electricity consumption, from purchased Renewable
Durable panel requires re-coating after 15 years. ProtectPlus
Energy Certificates (REC);
coating requires maintenance intervals every 25 years. The
• Waste processing up to the end-of-waste state or
conservative scenario, in which both coatings are applied, is
disposal of waste residues, during the production stage;
considered here, even though in reality we have application of
• Production of packaging material;
only one of them.
• Manufacturing of products and co-product.
The environmental impact of co-products from the steel and
End of Life
coal fired electricity production (slags, alumina and ashes
The End-of-life stage C1-C4 includes:
entering the system as inputs to the manufacturing) is
• C1 de-construction, demolition;
accounted for and economic allocation is applied. Recycled
• C2 transport to waste processing;
stone wool comes free of environmental burden, as it enters the
• C3 waste processing for reuse, recovery
product system as waste. Their transport to the factory is
• and/or recycling;
accounted for. Modules A1, A2 and A3 are declared as an
• C4 disposal.
aggregated module A1-A3.
These stages also include provision and all transport, provision
of all materials, products and related energy and water use.
Construction/Installation
Manual deconstruction is assumed for C1 and no impacts are
The Construction Stage A4-A5 includes:
assigned. The benefits from disposal (heat or electricity
• A4 transport to the building site
recovery) are assigned to module D.
• A5 installation to the building
3 Environmental Product Declaration - ROCKWOOL International A.S. - Rockpanel Durable & FS-Xtra
Module D includes reuse, recovery and/or recycling potentials The product system with the system boundaries is presented in
expressed as net loads and benefits. Here the loads from the the graph below:
packaging disposal in A5 and from electricity generation on
landfill are considered.
figure: product system with system boundaries Comparability
Basically, a comparison or an evaluation of EPD data is only
Geographic Representativeness possible if all the data sets to be compared were created
Land or region, in which the declared product system is according to EN 15804 and the building context, respectively
manufactured, used or handled at the end of the product´s the product-specific characteristics of performance, are taken
lifespan: Netherlands into account. The used software for the development of the
declaration was GaBi, version 8.0.1.257 by thinkstep.
LCA: Scenarios and additional technical information
Note: 1 kg of biogenic carbon is equivalent to 44/12 kg of CO 2. Name Value Unit
Re-application of
Information on
Rockpanel waterborne -
maintenance
The following technical information for the declared modules coating
can be used for scenario development in a building context.
Maintenance cycle 3 Number/RSL
Transport to the building site (A4) Information on Re-application of
Name Value Unit maintenance (2) ProtectPlus coating
Litres of fuel - l/100km Maintenance cycle
2 Number/RSL
Transport distance 353 km (2)
Capacity utilisation (including empty runs) 85 %
Gross density of products transported 1050 kg/m3
Installation into the building (A5) Reference service life
Name Value Unit
Electricity consumption - kWh
Material loss 5 %
Maintenance (B2)
4 Environmental Product Declaration - ROCKWOOL International A.S. - Rockpanel Durable & FS-Xtra
Name Value Unit End of life (C1 - C4)
Reference service life
Name Value Unit
(according to ISO 60 a
Landfilling 8.4 kg
15686-1, -2, -7 and -8)
Transport to landfill 50 km
According to product standards:
Utilization rate 50 %
EAD 090001-01-0404
“Prefabricated compressed
Declared product mineral wool boards with
properties (at the gate) organic or inorganic finish and -
and finishes with specified fastening system”;
According to Accelerated Reuse, recovery and/or recycling potentials (D), relevant
durability testing report from scenario information
Bouw Technologie Any declared benefits and loads from net flows leaving the
Design application product system that have not been allocated as co-products
parameters (if instructed See installation guidelines. and that have passed the end-of-waste state are included in
by the manufacturer), Installation to be conducted in module D. Such declared benefits can occur in stages A5 and
including the references accordance with manufacturers - C4. The generated energy, such as heat and electricity from
to the appropriate guidelines and the appropriate waste incineration of packaging is assigned to module D. The
practices and application Declaration of Performance benefits are calculated using current average substitution
codes processes. The heat is credited for with heat from natural gas.
It is assumed that the The electricity is credited for with the specific country’s
An assumed quality of manufacturer’s instructions are electricity mix. This is also applied for materials that are
work, when installed in clear and followed. In case of landfilled as the benefits from electricity production from landfill
accordance with the any uncertainty the - gas recovery are included in module D.
manufacturer’s
manufacturer should be
instructions
contacted for instructions
Outdoor environment,
(for outdoor
Product is designed for outdoor
applications), e.g.
application. The performance of
weathering, pollutants, -
the product is declared in the
UV and wind exposure,
Declaration of Performance.
building orientation,
shading, temperature
Indoor environment (for
indoor applications), e.g. Product is primarily designed for
-
temperature, moisture, outdoor application
chemical exposure
No usage conditions, except if
Usage conditions, e.g. specifically stated on the product
frequency of use, or in the Declaration of -
mechanical exposure Performance. Please follow the
manufacturer’s guidelines.
Maintenance e.g. The boards should be cleaned
required frequency, type occasionally with a cleaning
and quality and solution such as car shampoo or -
replacement of an all-purpose cleaner. Please
components refer to manufacturer guidelines.
5 Environmental Product Declaration - ROCKWOOL International A.S. - Rockpanel Durable & FS-Xtra
LCA: Results
DESCRIPTION OF THE SYSTEM BOUNDARY (X = INCLUDED IN LCA; MND = MODULE NOT DECLARED; MNR = MODULE NOT
RELEVANT)
Benefits and
Construction loads beyond
Product stage Use stage End of life stage
process stage the system
boundaries
la ire ta m w a Ry lp p u s tro p s n a rT g n iru tc a fu n a M e h t m o rf tro p s n a rTe tis e h t o t e ta g y lb m e s s A e s U e c n a n e tn ia M ria p e R tn e m e c a lp e R tn e m h s ib ru fe R y g re n e la n o ita re p Oe s u re ta w la n o ita re p Oe s u n o itc u rts n o c -e Dn o itilo m e d tro p s n a rT g n is s e c o rp e ts a W la s o p s iD -e s u e R-y re v o c e R-g n ilc y c e Rla itn e to p
A1 A2 A3 A4 A5 B1 B2 B3 B4 B5 B6 B7 C1 C2 C3 C4 D
X X X X X MND X MNR MNR MNR X X X X X X X
RESULTS OF THE LCA - ENVIRONMENTAL IMPACT according to EN 15804+A1: 1 m² Rockpanel Durable 8 mm
Parameter Unit A1-A3 A4 A5 B2 B6 B7 C1 C2 C3 C4 D
GWP kg CO 2 eq 1.43E+01 2.1E-01 1.46E+00 2.47E+00 0 0 0 3.15E-02 0 2.46E-01 -3.32E-01
kg CFC11
ODP 8.15E-08 3.49E-17 5E-09 2.21E-14 0 0 0 5.21E-18 0 7.57E-16 2.49E-13
eq
AP kg SO 2 eq 6.46E-02 1.78E-04 3.47E-03 1.02E-02 0 0 0 2.87E-05 0 7.86E-04 -1.14E-03
EP kg PO 43 eq 2.23E-02 3.93E-05 1.2E-03 7.81E-04 0 0 0 6.47E-06 0 1.27E-04 -1.01E-04
POCP kg Ethen eq 4.34E-03 6.68E-07 2.54E-04 9.37E-04 0 0 0 -7.88E-07 0 8.77E-05 -1.42E-04
ADPE kg Sb eq 1.03E-05 1.63E-08 5.16E-07 2.96E-06 0 0 0 2.43E-09 0 4.77E-08 -4.07E-08
ADPF MJ 1.72E+02 2.86E+00 9.52E+00 4.62E+01 0 0 0 4.27E-01 0 1.87E+00 -8.84E+00
GWP = Global warming potential; ODP = Depletion potential of the stratospheric ozone layer; AP = Acidification potential of land and water; EP =
Eutrophication potential; POCP = Formation potential of tropospheric ozone photochemical oxidants; ADPE = Abiotic depletion potential for non-fossil
resources; ADPF = Abiotic depletion potential for fossil resources
RESULTS OF THE LCA - INDICATORS TO DESCRIBE RESOURCE USE according to EN 15804+A1: 1 m² Rockpanel Durable 8
mm
Parameter Unit A1-A3 A4 A5 B2 B6 B7 C1 C2 C3 C4 D
PERE MJ 9.27E+01 1.67E-01 8.59E+00 5.1E+00 0 0 0 2.49E-02 0 2.39E-01 -2.81E+00
PERM MJ 4.26E+00 0 -3.54E+00 0 0 0 0 0 0 0 0
PERT MJ 9.7E+01 1.67E-01 5.05E+00 5.1E+00 0 0 0 2.49E-02 0 2.39E-01 -2.81E+00
PENRE MJ 1.41E+02 2.87E+00 1.02E+01 5.02E+01 0 0 0 4.29E-01 0 1.94E+00 -9.34E+00
PENRM MJ 3.72E+01 0 -1.62E-01 0 0 0 0 0 0 0 0
PENRT MJ 1.78E+02 2.87E+00 1E+01 5.02E+01 0 0 0 4.29E-01 0 1.94E+00 -9.34E+00
SM kg 5.49E+00 0 2.74E-01 0 0 0 0 0 0 0 -5.49E+00
RSF MJ 0 0 0 0 0 0 0 0 0 0 0
NRSF MJ 1.51E+01 0 7.53E-01 0 0 0 0 0 0 0 0
FW m3 1.57E-02 2.58E-04 1.76E-03 1.36E-02 0 0 0 4.21E-05 0 4.76E-04 -3.97E-03
PERE = Use of renewable primary energy excluding renewable primary energy resources used as raw materials; PERM = Use of renewable primary
energy resources used as raw materials; PERT = Total use of renewable primary energy resources; PENRE = Use of non-renewable primary energy
excluding non-renewable primary energy resources used as raw materials; PENRM = Use of non-renewable primary energy resources used as raw
materials; PENRT = Total use of non-renewable primary energy resources; SM = Use of secondary material; RSF = Use of renewable secondary fuels;
NRSF = Use of non-renewable secondary fuels; FW = Use of net fresh water
RESULTS OF THE LCA – WASTE CATEGORIES AND OUTPUT FLOWS according to EN 15804+A1:
1 m² Rockpanel Durable 8 mm
Parameter Unit A1-A3 A4 A5 B2 B6 B7 C1 C2 C3 C4 D
HWD kg 5.58E-07 1.6E-07 3.94E-08 7.49E-08 0 0 0 2.4E-08 0 3.16E-08 4.21E-09
NHWD kg 7.69E-01 2.34E-04 5.13E-01 6.79E-01 0 0 0 3.49E-05 0 8.55E+00 5.62E-01
RWD kg 1.33E-03 3.9E-06 1.36E-04 1.58E-03 0 0 0 5.82E-07 0 2.6E-05 -1.71E-05
CRU kg 0 0 0 0 0 0 0 0 0 0 0
MFR kg 0 0 1.65E-01 0 0 0 0 0 0 0 0
MER kg 0 0 0 0 0 0 0 0 0 0 0
EEE MJ 0 0 6.99E-01 0 0 0 0 0 0 4.41E-02 0
EET MJ 0 0 2.08E+00 0 0 0 0 0 0 0 0
HWD = Hazardous waste disposed; NHWD = Non-hazardous waste disposed; RWD = Radioactive waste disposed; CRU = Components for re-use;
MFR = Materials for recycling; MER = Materials for energy recovery; EEE = Exported electrical energy; EET = Exported thermal energy
References
EN 15804 works — Environmental Product Declarations — Core rules for
EN 15804:2012-04+A1 2013, Sustainability of construction the product category of construction products.
6 Environmental Product Declaration - ROCKWOOL International A.S. - Rockpanel Durable & FS-Xtra
July 2019.
ISO 14025
DIN EN ISO 14025:2011-10, Environmental labels and ETA-13/0340
declarations — Type III environmental declarations — European Technical Assessment ETA-13/0340 of 2018-01-18,
Principles and procedures. for ROCKPANEL A2 (FS-Xtra) 9 mm finish Colours/Rockclad,
Rockpanel A2 (FS-Xtra) 9 mm finish Structures and Rockpanel
IBU 2016 A2 (FS-Xtra) 9 mm finish ProtectPlus, available via
Institut Bauen und Umwelt e.V.: General Programme http://static.rockwool.com/globalassets/rockpanel/documentation/european-
Instructions for the Preparation of EPDs at the Institut Bauen echnical-assesments/rockpanel_eta_130340.pdf, accessed:
und Umwelt e.V. Version 1., Berlin: Institut Bauen und Umwelt July 2019.
e.V., 2016.
www.ibu-epd.com ETA-13/0648
ECHA PR/19/12 European Technical Assessment ETA-13/0648 of 02/11/2015,
The Candidate List of substances of very high concern, for Rockpanel Natural Durable 8 mm and 10 mm Rockpanel
available via https://echa.europa.eu/nl/-/four-new-substances- Natural Xtreme 8 mm and 10 mm, available via
added-to-the-candidate-list, accessed October 2019 https://www.rockpanel.fr/siteassets/documentation/rockpanel-
eta/rockpanel_eta_130648.pdf, accessed: July 2019.
ISO 12572:2016
ISO 12572:2016, Hygrothermal performance of building ETA-18/0883
materials and products – Determination of water vapour European Technical Assessment ETA-18/0883 for Rockpanel
transmission properties – Cup method. Premium A2, available via.
https://www.rockpanel.co.uk/resources/certificates/, accessed
EN 310 August 2019.
EN 310:1993, Wood-based panels — Determination of modulus
of elasticity in bending and of bending strength. EUCEB
Website of European Certification Board for mineral wool
EN 323 products: http://www.euceb.org/ [Accessed: July 2019].
EN 323:1993, Wood-based panels — Determination of density.
GaBi ts
EN 438-2 Leinfelden - Echterdingen GaBi Software - System and
EN 438-2:2016+A1:2018, High-pressure decorative laminates Database for Life cycle Engineering. Thinkstep AG, LBP,
(HPL) — Sheets based on thermosetting resins (usually called University of Stuttgart and PE. Program version
laminates) — Determination of properties. 8.0.1.257,database schema 8006 International, 2011.
EN 1058 GaBi-Dokumentation
EN 1058:2009, Wood-based panels —. Determination of Thinkstep AG: GaBi 6 life cycle inventory data documentation,
characteristic 5-percentile values and characteristic mean 2018.
value. http://www.gabisoftware.com/support/gabi/gabi-6-
lcidocumentation [Accessed: July 2019].
EN 3120
EN 3120:2012, Aerospace series — Titanium alloy TI-P64003 IBU PCR - Part A
— Cold worked and stress relieved — Seamless tube for Calculation rules for the Life Cycle Assessment and
pressure systems 4 mm ≤ D ≤ 51 mm, 690 MPa ≤ Rm ≤ 1 030 Requirements on the Background Report, version 1.6, Institut
MPa. Bauen und Umwelt e.V., www.bau-umwelt.com, Juli 2019.
EN 10456 IBU 2017, PCR, Part B
EN ISO 10456:2007, Building materials and products — PCR- Part B: Requirements on the EPD for mineral insulating
Hygrothermal properties — Tabulated design values and products, Institut Bauen und Umwelt e.V., www.bau-
procedures for determining declared and design thermal umwelt.com, Januar 2019.
values.
Regulation (EC) No 305/2011
ETA-07/0141 Regulation (EC) No 305/2011 of the European Parliament and
European Technical Assessment ETA-07/0141 of 15/12/2014, of the council of 9 March 2011 laying down harmonised
for Rockpanel Durable 8 mm finish Colours/Rockclad and conditions for the marketing of construction products and
Rockpanel Durable 8 mm finish ProtectPlus, available via repealing Council Directive 89/106/EEC. Available at:
https://www.rockpanel.fr/siteassets/documentation/rockpanel- https://eur-lex.europa.eu/legal-content/EN/TXT/?uri=celex
eta/rockpanel_eta_070141.pdf, accessed: July 2019. %3A32011R0305.
ETA-08/0343 Regulation (EC) No 1272/2008 - REACH
European Technical Assessment ETA-08/0343 of 16/09/2014, Regulation (EC) No 1272/2008 of the European Parliament and
for Rockpanel Durable 6 mm finish Colours / Rockclad, of the council of 16 December 2008 on classification, labeling
available via and packaging of substances and mixtures. Available at:
http://static.rockwool.com/globalassets/rockpanel/documentation/europehattnp-s://eurlex.europa.eu/legalcontent/EN/TXT/?
echnical-assesments/rockpanel_eta_080343.pdf, accessed: uri=celex:32008R1272 [Accessed: July 2019].
7 Environmental Product Declaration - ROCKWOOL International A.S. - Rockpanel Durable & FS-Xtra
Publisher
Institut Bauen und Umwelt e.V. +49 (0)30 3087748- 0
Hegelplatz 1 info@ibu-epd.com
10117 Berlin www.ibu-epd.com
Germany
Programme holder
Institut Bauen und Umwelt e.V. +49 (0)30 3087748- 0
Hegelplatz 1 info@ibu-epd.com
10117 Berlin www.ibu-epd.com
Germany
Author of the Life Cycle Assessment
ROCKWOOL International A/S +45 46 56 03 00
Hovedgaden 584 info@rockwool.com
2640 Hedehusene www.rockwoolgroup.com
Denmark
Owner of the Declaration
ROCKWOOL International A/S +45 46 56 03 00
Hovedgaden 584 info@rockwool.com
2640 Hedehusene www.rockwoolgroup.com
Denmark
8 Environmental Product Declaration - ROCKWOOL International A.S. - Rockpanel Durable & FS-Xtra
