ENVIRONMENTAL PRODUCT DECLARATION
as per ISO 14025 and EN 15804+A2
Owner of the Declaration ARGE – The European Federation of Locks and Building Hardware Manufacturers
Publisher Institut Bauen und Umwelt e.V. (IBU)
Programme holder Institut Bauen und Umwelt e.V. (IBU)
Declaration number EPD-ARG-20230549-IBG1-EN
Issue date 02.04.2024
Valid to 01.04.2029
Sliding door hardware
ARGE – The European Federation of Locks
and Building Hardware Manufacturers
This EPD is valid only for products supplied by an ARGE EPD licence holder.
www.ibu-epd.com | https://epd-online.com
1. General Information
ARGE – The European Federation of Locks Sliding door hardware
and Building Hardware Manufacturers
Programme holder Owner of the declaration
IBU – Institut Bauen und Umwelt e.V. ARGE – The European Federation of Locks and Building Hardware
Hegelplatz 1 Manufacturers
10117 Berlin Offerstraße 12
Germany 42551 Velbert
Germany
Declaration number Declared product / declared unit
EPD-ARG-20230549-IBG1-EN 1 kg sliding door hardware
This declaration is based on the product category rules: Scope:
Building Hardware products, 01.08.2021 This ARGE EPD covers hardware systems for sliding doors, sliding corner
(PCR checked and approved by the SVR) doors, sliding folding doors and sliding gates used for buildings as well as
mechanisms used to support doors of varying materials and allow their
opening and closing by a sliding action. It does not include sliding folding
Issue date windows or door height windows. The reference product used to calculate
the impact this product group has on the environment is an item of sliding
02.04.2024
door hardware composed primarily of aluminium and has been selected for
the LCA (Life Cycle Assessment) because it is the product with the highest
impact for 1 kg of product. A validity scope analysis has also been carried
Valid to
out to determine the limiting factors for sliding door gear covered by this
01.04.2029 EPD. In a preliminary study (simplified LCA), it has been confirmed that
this EPD represents the worst-case condition and it can therefore be used
to cover all sliding door hardware manufactured in Europe by ARGE
member companies.
The owner of the declaration shall be liable for the underlying information
and evidence; the IBU shall not be liable with respect to manufacturer
information, life cycle assessment data and evidences.
The EPD was created according to the specifications of EN 15804+A2. In
the following, the standard will be simplified as EN 15804.
Verification
Dipl.-Ing. Hans Peters The standard EN 15804 serves as the core PCR
(Chairman of Institut Bauen und Umwelt e.V.)
Independent verification of the declaration and data according to ISO
14025:2011
internally X externally
Florian Pronold Dr. Matthew Fishwick,
(Managing Director Institut Bauen und Umwelt e.V.) (Independent verifier)
1 Environmental Product Declaration - ARGE – The European Federation of Locks and Building Hardware Manufacturers - Sliding door hardware
2. Product
the ring-opening polymerisation of caprolactam. Components
2.1 Product description/Product definition
made of Nylon 6 are formed by injection moulding or other
This EPD covers sliding door hardware intended to be used for thermal forming processes.
buildings. The sample group used to calculate the LCA data for
this EPD includes all functional hardware necessary to move a Steel is produced by combining iron with carbon as well as
sliding door safely. other elements depending on the desired characteristics.
For the application and use the respective national provisions Components made of steel are formed by stamping or other
apply. types of mechanical processing.
2.2 Application
1) This product/article/at least one partial article contains
These products are designed to be integrated into door and substances listed in the ECHA candidate list (date: 14.06.2023)
gate assemblies consisting of various materials and used for exceeding 0.1 percentage by mass: Certain components may
various applications. Their purpose is to ensure the fastening of contain small amounts of lead (CAS no. 7439-92-1) as an
the door or gate and to open and close it safely. They may be alloying element.
used for either interior or exterior doors or for gates.
2) This product/article/at least one partial article contains other
2.3 Technical Data
cancerogenic, mutagenic, reprotoxic (CMR) substances in
Ideally, products should comply with a suitable technical
categories 1A or 1B which are not on the ECHA candidate list,
specification. EN 1527:2019+A1:2021,
exceeding 0.1 percentage by mass: no.
Building hardware – Hardware for sliding doors and folding
doors – Requirements and test methods and EN 13126-
3) Biocide products were added to this construction product or it
15:2019, Building hardware - Hardware for windows and door
has been treated with biocide products (this then concerns a
height windows - Requirements and test methods - Part 15:
treated product as defined by the (EU) Ordinance on Biocide
Rollers for horizontal sliding and hardware for sliding folding
Products No. 528/2012): no.
windows are examples of such specifications and some
products will comply with them. The relevant grading structure 2.6 Manufacture
is shown in the following table:
The manufacture of sliding door hardware usually follows a 3-
Grading structure according to EN 1527: step process:
Name Value Unit 1. Manufacture of the components: this step may include
Category of door 1 - 3 surface treatment in the factory or by external
contractors.
Door mass 1 - 4
2. Pre-assembly of modules (in the factory).
Size of Test Panel Used 0 - 4
3. Final assembly (in the factory).
Corrosion resistance 0 - 5
Slam test resistance 1 - 3 2.7 Environment and health during manufacturing
Regular measurements of air quality and noise levels are
Horizontal static load test resistance 1 - 3
carried out by the manufacturers, the ARGE member
Static load test resistance 0, 1
companies. The results shall be within the mandatory safety
Initial friction maximum permitted value 1 - 3
levels. In areas where employees are exposed to chemical
Durability 1 - 6 products, the required protective clothing and technical
Performance data of the product with respect to its protective devices shall be provided. Regular health checks are
characteristics in accordance with the relevant technical mandatory for employees in production facilities.
provision (no CE-marking).
2.8 Product processing/Installation
2.4 Delivery status The installation of the products may vary depending on the type
of door or gate and the specific situation, but the products shall
The products are sold by unit. Deliveries of individual items are
not require energy consumption for installation.
possible but are an exception. Standard deliveries comprise a
larger quantity of sliding door hardware, as it is marketed as
2.9 Packaging
"B2B" product and not to end-users.
Normally, each individual product is packed in paper or
2.5 Base materials/Ancillary materials cardboard. These individual products are then packed in a
cardboard box and stacked on wooden pallets for transport to
Composition of product analysed for this EPD:
the customer.
The values given are for the product analysed for this EPD.
Waste from product packaging is collected separately for waste
Ranges of the values for other products covered by the validity
scope analysis are given in brackets. disposal (including recycling).
Name Value Unit 2.10 Condition of use
Aluminium (0.00% – 97.20%) 97.2 % Once installed, the products shall require no servicing during
Nylon 6 (0.00% – 8.28%) 2.5 % their expected service lives. There shall be no consumption of
Steel (0.31% – 100.00%) 0.31 % water or energy linked to their use, and they shall not cause
any emissions.
Aluminium is a non-ferrous metal produced from bauxite by
the Bayer process. Components made of aluminium are 2.11 Environment and health during use
manufactured by extrusion or other types of mechanical No environmental damage or health risks are to be expected
processing. during normal conditions of use.
Nylon 6 is a polymer, in particular polyamide. It is formed by
2 Environmental Product Declaration - ARGE – The European Federation of Locks and Building Hardware Manufacturers - Sliding door hardware
Mechanical destruction
2.12 Reference service life Mechanical destruction of the declared product shall not
The reference service life is 30 years under normal working materially alter its composition or have any adverse effect on
conditions. This corresponds to passing a mechanical the environment.
endurance test of 100.000 cycles as specified in the EN 1527
and EN 15706. The reference service life is dependent on the 2.14 Re-use phase
actual frequency of use and environmental conditions. It is Removal of sliding door hardware (for re-use or recycling) shall
required that installation, as well as maintenance of the have no adverse effect on the environment.
product, must be done in line with instructions provided by the
manufacturer. 2.15 Disposal
Sliding door gear should be re-cycled wherever possible,
2.13 Extraordinary effects providing that there is no adverse effect on the environment .
Fire The waste code in accordance with the European Waste Code
There are no specific fire resistance requirements. is 17 04 07.
Water 2.16 Further information
The declared product is intended to be used for a building Details of all types and variants can be found on the
under normal conditions (indoor or outdoor use) It shall not emit manufacturers' websites. The respective website addresses are
hazardous substances in the event of flooding. available at https://arge.org.
3. LCA: Calculation rules
• when a material is sent for, recycling, generic transport
3.1 Declared Unit
and electric consumption of a shredder is taken into
The declared unit for all products covered by ARGE EPD is 1
account (corresponding to the process 'Grinding,
kg (of product). Since individual products will rarely weigh
metals'). Only then, is the material considered to have
exactly 1 kg it is necessary to establish the exact weight of the
attained the 'end-of-waste' state.
product and then use this as a correction factor to determine
• each type of waste is modelled as a transport to the
the true values for 1 kg of product in the tables (Section 5).
treatment site with a distance of 30 km. Parts sent for
recycling include electricity consumption (grinding) and
Declared unit a flow ('Materials for recycling, unspecified').
Name Value Unit
3.3 Estimates and assumptions
Declared unit 1 kg
The LCA data of the declared product had been calculated
Mass of declared product 3.92 kg
using the production data of an ARGE member company that
Raw density 1 kg/m3 manufactures 6 different products. The company had been
chosen by ARGE as being representative by virtue of their
production processes and market share. The sliding door
3.2 System boundary hardware chosen as representative for this calculation follows
Type of the EPD: "cradle to gate with options, with modules C1 the "worst-case" principle as explained under 6 LCA
– C4, and module D (A1-A3, C1-C3, D and additional interpretation.
modules)"
3.4 Cut-off criteria
The cut-off criteria considered are 1% of renewable and non-
The analysis of the product life cycle includes the production
renewable primary energy usage and 1% of the total mass of
and transport of the raw materials, the manufacture of the
that unit process. The total neglected input flows per module
product and the packaging materials which are declared in
shall be a maximum of 5% of energy usage and mass.
modules A1-A3.
Losses during production are considered as waste and are sent
For this study, all input and output flows have been considered
for recycling. No recycling processes are taken into account
at 100%, including raw materials as per the product
except for transport and electricity consumption for grinding the
composition provided by the manufacturer and packaging of
metals. When recycled metals are used as raw material only
raw materials as well as the final product. Energy and water
their transformation process is taken into account and not the
consumptions have also been considered at 100% according to
extraction of the raw material.
the data provided.
A4 module represents the transport of the finished sliding door
gear to the installation site.
With the approach chosen, no significant environmental
There is no waste associated with the installation of the
impacts are known to have been cut off.
product. The A5 module therefore represents only the disposal
of the product packaging.
3.5 Background data
The End-of-Life (EoL) stages are also considered. The
For the life cycle modelling of the considered product, all
transportation to the EoL disposal site is taken into account in
relevant background datasets are taken from ecoinvent v3.8
module C2. Module C4 covers the disposal of the locks. Module
(system model: cut-off by classification).
C3 covers the recycling of the individual elements according to
European averages, with the remaining waste divided between 3.6 Data quality
incineration and landfill. Such a mixed scenario is declared due
The objective of this evaluation is to evaluate the environmental
to the complex material mix of the product and the dependency
impacts generated by the products throughout their entire life
of the EoL-route on the EoL-route of the product the sliding
cycles. To this end, ISO 14040, ISO 14044 and EN 15804 have
door hardware has been integrated into.
been met regarding the quality of data on the following different
In practice, the end of life has been modelled as follows:
criteria:
3 Environmental Product Declaration - ARGE – The European Federation of Locks and Building Hardware Manufacturers - Sliding door hardware
year 2022.
Time: The life cycle inventory data used come from:
3.8 Geographic Representativeness
• Data collected specifically for this study on the ARGE
Land or region, in which the declared product system is
member companies' manufacturing sites. Datasets are
manufactured, used or handled at the end of the product´s
based on 1-year averaged data (time period: January
lifespan: Europe
2013 to December 2013 considered representative for
2022).
• In the absence of collected data, generic data from the 3.9 Allocation
ecoinvent v3.8 database have been used. This is
The products are produced in one production site. All data were
updated regularly and is representative of current
provided by the manufacturer of the products per unit and then
processes (the entire database having been updated in
divided by the mass of the product to give a value per kg of
2021).
product produced.
Geography: Data come from production sites of the ARGE
member companies. Generic data come from the ecoinvent
The assumptions relating to the EoL of the product are
database, representative for European production processes.
described in the section System Boundaries.
Technology: Material shaping technologies are based on 3.10 Comparability
European technology in the case of the use of generic data. Basically, a comparison or an evaluation of EPD data is only
possible if all the data sets to be compared were created
A total of 6 typical products (based on sales figures) have been according to EN 15804 and the building context, respectively
evaluated, and the worst-case results are used in the tables. the product-specific characteristics of performance, are taken
into account.
3.7 Period under review
ecoinvent v3.8 (system model: cut-off by classification) has
The data of the LCA is based on the annual production data of
been used as the background database.
an ARGE member from 2013, considered representative for the
4. LCA: Scenarios and additional technical information
It is assumed that a 16–32-ton truck is used to transport the
Characteristic product properties of biogenic carbon
product:
- Transport to shredding facility for metal recovery: 150 km
Information on the biogenic carbon content at factory gate - Transport to municipal waste incineration plant: 50 km
- Transport to landfill: 30 km
Note: 1 kg of biogenic carbon is equivalent to 44/12 kg of CO .
2
Name Value Unit Reuse, recovery and/or recycling potentials (D), relevant
kg scenario information
Biogenic carbon content in product 0
C Module D contains the benefits and loads beyond the system
Biogenic carbon content in accompanying kg boundary related to the recycling of metals, which result from
0.0354
packaging C the treatment of recycled materials from the point of end-of-
waste status to the point of substitution (as costs) and the
substitution of primary resources (as benefits).
The following information is the basis of the declared modules
within the LCA in this EPD.
According to EN 16710, clause 6.4.3.3: 'In module D
Transport to the building site (A4) substitution effects are calculated only for the resulting net
Name Value Unit output flow.
Litres of fuel 25.8 l/100km
For building hardware, the following rules apply for the
Transport distance 3500 km
quantification of net output flows:
- all production scrap and cuttings leave modules A1-B3 as
Installation into the building (A5)
sorted scrap without allocated burdens from primary production;
Name Value Unit
the corresponding amounts are declared as material for
Material loss 0.144 kg recycling (MFR);
- net amounts of a metal leaving the product system are
quantified as the material for recycling leaving modules A1-C4
Reference service life minus the input of secondary scrap (secondary material, SM) to
Name Value Unit the product system;
Reference service life 30 a - in the case of brass and zinc alloys, which are composed of
two different constituting metals, no difference shall be made
Test cycles over RSL (EN 1527, EN 15706) 100'000 cycles
between the input of secondary constituting metals (Cu and Zn;
End of life (C1-C4) Cu and Sn) and its alloys (CuZn; CuSn).
Negative net output flows have been considered in the
Name Value Unit
quantification of module D.
Collected separately waste type 1 kg
It also includes the benefits and loads related to 'exported
Recycling 0.472 kg energy electricity' and 'exported energy heat' resulting from the
Energy recovery 0.243 kg energy recovery from plastic wastes in a municipal waste
Landfilling 0.285 kg incineration plant as modelled in Modules A3, A5 and C4.
4 Environmental Product Declaration - ARGE – The European Federation of Locks and Building Hardware Manufacturers - Sliding door hardware
5. LCA: Results
In Table 1 "Description of the system boundary", the declared modules are indicated with an "X"; all modules that are not declared
within the EPD but where additional data are available are indicated with "MND". Those data can also be used for building assessment
scenarios. The values are declared with three valid digits in exponential form.
DESCRIPTION OF THE SYSTEM BOUNDARY (X = INCLUDED IN LCA; MND = MODULE OR INDICATOR NOT DECLARED; MNR
= MODULE NOT RELEVANT)
Benefits and
Construction loads beyond
Product stage Use stage End of life stage
process stage the system
boundaries
la ire wta am R y lp p u s tro p s n a rT g n iru tc a fu n a M tro p s nm ae o rh r
T
f te tis e h t o t e ta g y lb m e s s A e s U e c n a n e tn ia M ria p e R tn e m e c a lp e R tn e m h s ib ru fe R la n o ity ag rr ee pn Oe e s u la n o ita r re et pa Ow e s u n o itc u rts n eo Dc -n o itilo m e d tro p s n a rT g n is s ee tsc ao Wrp la s o p s iD e s u e R- y re v o c e R- g n ilc y c e R- la itn e to p
A1 A2 A3 A4 A5 B1 B2 B3 B4 B5 B6 B7 C1 C2 C3 C4 D
X X X X X MND MND MNR MNR MNR MND MND X X X X X
RESULTS OF THE LCA - ENVIRONMENTAL IMPACT according to EN 15804+A2: 1 kg of sliding door gear
Parameter Unit A1-A3 A4 A5 C1 C2 C3 C4 D
GWP-total kg CO2 eq 1.7E+01 6.21E-01 1.43E-01 0 1.65E-02 3.67E-03 2.56E-02 -6.52E+00
GWP-fossil kg CO2 eq 1.71E+01 6.21E-01 1.33E-02 0 1.65E-02 3.66E-03 2.56E-02 -6.49E+00
GWP-biogenic kg CO2 eq -1.3E-01 0 1.3E-01 0 0 0 0 0
GWP-luluc kg CO2 eq 4.66E-02 2.48E-04 8.53E-07 0 6.59E-06 9.13E-06 3.39E-06 -2.42E-02
ODP kg CFC11 eq 6.55E-07 1.44E-07 4.89E-10 0 3.82E-09 1.86E-10 1.63E-09 -2.15E-07
AP mol H+ eq 1.16E-01 1.76E-03 7.88E-06 0 4.68E-05 1.89E-05 4.74E-05 -4.25E-02
EP-freshwater kg P eq 5.65E-04 4.43E-06 1.63E-08 0 1.17E-07 4.11E-07 8.81E-08 -2.37E-04
EP-marine kg N eq 1.79E-02 3.5E-04 2.15E-06 0 9.3E-06 2.42E-06 1.83E-05 -6.3E-03
EP-terrestrial mol N eq 1.97E-01 3.9E-03 2.36E-05 0 1.04E-04 2.79E-05 1.91E-04 -6.94E-02
kg NMVOC
POCP 5.73E-02 1.5E-03 7.53E-06 0 3.98E-05 7.64E-06 5.56E-05 -2.06E-02
eq
ADPE kg Sb eq 1.1E-04 2.2E-06 7.63E-09 0 5.84E-08 8.87E-09 2.87E-08 3.27E-05
ADPF MJ 1.67E+02 9.41E+00 3.26E-02 0 2.5E-01 7.76E-02 1.26E-01 -5.83E+01
m3 world eq
WDP 2.62E+00 2.86E-02 1.43E-04 0 7.6E-04 8.67E-04 -1.14E-03 -8.94E-01
deprived
GWP = Global warming potential; ODP = Depletion potential of the stratospheric ozone layer; AP = Acidification potential of land and water; EP =
Eutrophication potential; POCP = Formation potential of tropospheric ozone photochemical oxidants; ADPE = Abiotic depletion potential for non-fossil
resources; ADPF = Abiotic depletion potential for fossil resources; WDP = Water (user) deprivation potential)
RESULTS OF THE LCA - INDICATORS TO DESCRIBE RESOURCE USE according to EN 15804+A2: 1 kg of sliding door gear
Parameter Unit A1-A3 A4 A5 C1 C2 C3 C4 D
PERE MJ 1.79E+01 1.32E-01 -6.57E-02 0 3.51E-03 1.47E-02 1.39E-02 -7.83E+00
PERM MJ 8.04E-01 0 -6.57E-01 0 0 0 0 0
PERT MJ 1.87E+01 1.32E-01 -7.23E-01 0 3.51E-03 1.47E-02 1.39E-02 -7.83E+00
PENRE MJ 1.66E+02 9.41E+00 1.95E-01 0 2.5E-01 7.83E-02 3.91E-01 -5.85E+01
PENRM MJ 7.38E-01 0 -1.63E-01 0 0 0 -2.65E-01 0
PENRT MJ 1.67E+02 9.41E+00 3.26E-02 0 2.5E-01 7.83E-02 1.26E-01 -5.85E+01
SM kg 3.93E-01 0 0 0 0 0 0 0
RSF MJ 0 0 0 0 0 0 0 0
NRSF MJ 0 0 0 0 0 0 0 0
FW m3 1.08E-01 9.98E-04 1.4E-05 0 2.65E-05 5E-05 2.22E-04 -4.36E-02
PERE = Use of renewable primary energy excluding renewable primary energy resources used as raw materials; PERM = Use of renewable primary
energy resources used as raw materials; PERT = Total use of renewable primary energy resources; PENRE = Use of non-renewable primary energy
excluding non-renewable primary energy resources used as raw materials; PENRM = Use of non-renewable primary energy resources used as raw
materials; PENRT = Total use of non-renewable primary energy resources; SM = Use of secondary material; RSF = Use of renewable secondary fuels;
NRSF = Use of non-renewable secondary fuels; FW = Use of net fresh water
RESULTS OF THE LCA – WASTE CATEGORIES AND OUTPUT FLOWS according to EN 15804+A2:
1 kg of sliding door gear
Parameter Unit A1-A3 A4 A5 C1 C2 C3 C4 D
HWD kg 2.67E-03 2.46E-05 1E-07 0 6.52E-07 2.75E-08 2.09E-07 8.55E-04
NHWD kg 4.44E+00 4.95E-01 1.89E-03 0 1.31E-02 2.92E-04 3.66E-01 -1.59E+00
RWD kg 6.2E-04 1.36E-04 4.54E-07 0 3.61E-06 1.04E-06 1.65E-06 -1.8E-04
CRU kg 0 0 0 0 0 0 0 0
MFR kg 1.94E-01 0 8.09E-02 0 0 5.48E-01 0 0
MER kg 0 0 0 0 0 0 0 0
EEE MJ 0 0 9.2E-03 0 0 0 1.12E-02 0
5 Environmental Product Declaration - ARGE – The European Federation of Locks and Building Hardware Manufacturers - Sliding door hardware
EET MJ 0 0 6.09E-02 0 0 0 7.43E-02 0
HWD = Hazardous waste disposed; NHWD = Non-hazardous waste disposed; RWD = Radioactive waste disposed; CRU = Components for re-use;
MFR = Materials for recycling; MER = Materials for energy recovery; EEE = Exported electrical energy; EET = Exported thermal energy
RESULTS OF THE LCA – additional impact categories according to EN 15804+A2-optional:
1 kg of sliding door gear
Parameter Unit A1-A3 A4 A5 C1 C2 C3 C4 D
Disease
PM 1.37E-06 4.99E-08 1.76E-10 0 1.32E-09 5.04E-11 1.15E-09 -5.51E-07
incidence
IR kBq U235 eq 2.84E-01 4.09E-02 1.37E-04 0 1.08E-03 7.07E-04 6.78E-04 -6.74E-02
ETP-fw CTUe 4.46E+02 7.39E+00 2.74E-02 0 1.96E-01 3.9E-02 1.39E+02 -1.38E+02
HTP-c CTUh 2.24E-08 2.38E-10 1.33E-12 0 6.3E-12 1.04E-12 1.6E-11 -7.37E-09
HTP-nc CTUh 4.34E-07 7.46E-09 4.68E-11 0 1.98E-10 3.39E-11 2.47E-10 -1.24E-07
SQP SQP 4.12E+01 6.56E+00 2.2E-02 0 1.74E-01 1.19E-02 2.24E-01 -8.95E+00
PM = Potential incidence of disease due to PM emissions; IR = Potential Human exposure efficiency relative to U235; ETP-fw = Potential comparative
Toxic Unit for ecosystems; HTP-c = Potential comparative Toxic Unit for humans (cancerogenic); HTP-nc = Potential comparative Toxic Unit for humans
(not cancerogenic); SQP = Potential soil quality index
Disclaimer 1 – for the indicator 'Potential Human exposure efficiency relative to U235'. This impact category deals mainly with the
eventual impact of low-dose ionizing radiation on human health of the nuclear fuel cycle. It does not consider effects due to possible
nuclear accidents, occupational exposure or radioactive waste disposal in underground facilities. Potential ionizing radiation from the
soil, radon and from some construction materials is also not measured by this indicator.
Disclaimer 2 – for the indicators 'abiotic depletion potential for non-fossil resources', 'abiotic depletion potential for fossil resources',
'water (user) deprivation potential, deprivation-weighted water consumption', 'potential comparative toxic unit for ecosystems', 'potential
comparative toxic unit for humans – cancerogenic', 'Potential comparative toxic unit for humans - not cancerogenic', 'potential soil
quality index'. The results of this environmental impact indicator shall be used with care as the uncertainties on these results are high
as there is limited experience with the indicator.
6. LCA: Interpretation
6 Environmental Product Declaration - ARGE – The European Federation of Locks and Building Hardware Manufacturers - Sliding door hardware
Figure 1 illustrates the relative contributions of the different modules along the life cycle of the declared products.
are in the order of 20 % to 30 % of the impacts over the product
Figure 1: Environmental impacts of sliding door hardware life cycle (modules A1-A3) and relate basically to the recycling
along its life cycle of metals; module. Only for ADP elements, the negative net
amount of zinc leaving the product system leads to additional
The largest part of environmental impacts is caused during burdens in module D from the compensation of material losses
production (modules A1-A3); comparably small impacts are with primary production of zinc.
caused during the transport of the product to the construction
site (via the manufacturer of the product, which the sliding door A total of 6 typical products (based on sales figures) have been
gear has been integrated into). evaluated and the worst-case results are used in section 5 of
this EPD. In chapter 2.5, the tabulated range of relative weight
All the other modules related to the product life cycle are not per material ensures that the variability of results stays within
significant. +/- 40% of the declared values (assessed for the indicators
GWP, PENRT, and non-hazardous waste).
Benefits and burdens beyond the system boundary (module D)
7. Requisite evidence
No testing results are required by the PCR part B.
8. References
Product category rules of IBU
EN 17610
IBU (2021) EN 17610:2022, Building hardware - Environmental product
IBU (2021): General Instructions for the EPD Programme of the declarations - Product category rules complementary to EN
Institut Bauen und Umwelt e.V. (General Instructions for the 15804 for building hardware.
IBU EPD Programme). Version 2.0, Institut Bauen und Umwelt,
Berlin. ISO 14025
ISO 14025:2006-07, Environmental labels and declarations -
IBU (2021) Type III Environmental declarations - Principles and
IBU (2021): PCR Part A: Calculation rules for the life cycle procedures.
assessment and requirements on the project report according
to EN 15804+A2. Version 1.3., Institut Bauen und Umwelt, ISO 14044
Berlin. EN ISO 14044:2006-07, Environmental management - Life
cycle assessment - Requirements and guidance (ISO
IBU (2023) 14044:2006); German and English versions EN ISO
IBU (2023): PCR Part B: Requirements on the EPD for building 14044:2006.
hardware products, Institut Bauen und Umwelt, Berlin.
EN 1527
Standards and legal documents EN 1527:2019+A1:2021, Building hardware - Hardware for
sliding doors and folding doors - Requirements and test
EN 15804 methods.
EN 15804:2012+A2:2019+AC:2021, Sustainability of
construction works - Environmental product declarations - Core EN 13126-15
rules for the product category of construction products. EN 13126-15:2019
7 Environmental Product Declaration - ARGE – The European Federation of Locks and Building Hardware Manufacturers - Sliding door hardware
Building hardware – Hardware for windows and door height biocidal products.
windows – Requirements and test methods – Part 15: Rollers
for horizontal sliding and hardware for sliding folding windows. European List of Waste
Commission Decision of 3 May 2000 replacing Decision
EN 15706 94/3/EC establishing a list of wastes pursuant to Article 1(a) of
EN 15706:2009, Hardware for furniture - Strength and durability Council Directive 75/442/EEC on waste and Council Decision
of slide fittings for sliding doors and roll fronts. 94/904/EC establishing a list of hazardous waste pursuant to
Article 1(4) of Council Directive 91/689/EEC on hazardous
ISO 15686 waste (notified under document number C(2000) 1147).
ISO 15686:1, -2, -7 and -8. Service life planning (various parts).
Additional references
ECHA candidate list
Candidate List of substances of very high concern for BBSR 2017
Authorisation, published in accordance with Article 59(10) of the BBSR (2017): Nutzungsdauer von Bauteilen in
REACH Regulation. European Chemicals Agency, Brussels. Lebenszyklusanalysen nach Bewertungssystem Nachhaltiges
Bauen (BNB). Version vom 24.10.2017, Bundesinstitut für Bau-,
Ordinance on Biocide Products No. 528/2012 Stadt- und Raumforschung, Berlin.
REGULATION (EU) No 528/2012 OF THE EUROPEAN
PARLIAMENT AND OF THE COUNCIL of 22 May 2012 ecoinvent v3.8
concerning the making available on the market and use of http://www.ecoinvent.org
8 Environmental Product Declaration - ARGE – The European Federation of Locks and Building Hardware Manufacturers - Sliding door hardware
Publisher
Institut Bauen und Umwelt e.V. +49 (0)30 3087748- 0
Hegelplatz 1 info@ibu-epd.com
10117 Berlin www.ibu-epd.com
Germany
Programme holder
Institut Bauen und Umwelt e.V. +49 (0)30 3087748- 0
Hegelplatz 1 info@ibu-epd.com
10117 Berlin www.ibu-epd.com
Germany
Author of the Life Cycle Assessment
Dr. Frank Werner - Umwelt & Entwicklung + 41 (0)44 241 39 06
Kammelenbergstrasse 30 frank@frankwerner.ch
9011 St. Gallen http://www.frankwerner.ch/
Switzerland
Owner of the Declaration
ARGE – The European Federation of Locks and +49 (0)2051 9506 15
Building Hardware Manufacturers mail@arge.org
Offerstraße 12 www.arge.org
42551 Velbert
Germany
9 Environmental Product Declaration - ARGE – The European Federation of Locks and Building Hardware Manufacturers - Sliding door hardware
