ENVIRONMENTAL PRODUCT DECLARATION
as per ISO 14025 and EN 15804+A2
Owner of the Declaration ARGE – The European Federation of Locks and Building Hardware Manufacturers
Publisher Institut Bauen und Umwelt e.V. (IBU)
Programme holder Institut Bauen und Umwelt e.V. (IBU)
Declaration number EPD-ARG-20230546-IBG3-EN
Issue date 07.05.2024
Valid to 06.05.2029
Locks
ARGE – The European Federation of Locks
and Building Hardware Manufacturers
www.ibu-epd.com | https://epd-online.com
1. General Information
ARGE – The European Federation of Locks Locks
and Building Hardware Manufacturers
Programme holder Owner of the declaration
IBU – Institut Bauen und Umwelt e.V. ARGE – The European Federation of Locks and Building Hardware
Hegelplatz 1 Manufacturers
10117 Berlin Offerstraße 12
Germany 42551 Velbert
Germany
Declaration number Declared product / declared unit
EPD-ARG-20230546-IBG3-EN 1 kg of lock
This declaration is based on the product category rules: Scope:
Building Hardware products, 01.08.2021 This ARGE EPD covers locks used to secure doors, windows or shutters in
(PCR checked and approved by the SVR) buildings. The reference product used to calculate the impact this product
group has on the environment is a high security night latch composed
primarily of steel, Zamak and brass, and has been selected for the LCA
Issue date (Life Cycle Assessment) because it is the product with the highest impact
for 1 kg of product. A validity scope analysis has also been carried out to
07.05.2024
determine the limiting factors for locks covered by this EPD. In a
preliminary study (simplified LCA), it has been confirmed that this EPD
represents the worst-case condition and it can therefore be used to cover
Valid to
all locks manufactured in Europe by ARGE member companies.
06.05.2029 The owner of the declaration shall be liable for the underlying information
and evidence; the IBU shall not be liable with respect to manufacturer
information, life cycle assessment data and evidences.
The EPD was created according to the specifications of EN 15804+A2. In
the following, the standard will be simplified as EN 15804.
Verification
The standard EN 15804 serves as the core PCR
Independent verification of the declaration and data according to ISO
14025:2011
Dipl.-Ing. Hans Peters internally X externally
(Chairman of Institut Bauen und Umwelt e.V.)
Florian Pronold Dr. Matthew Fishwick,
(Managing Director Institut Bauen und Umwelt e.V.) (Independent verifier)
1 Environmental Product Declaration - ARGE – The European Federation of Locks and Building Hardware Manufacturers - Locks
2. Product
larger quantity of locks, as they are marketed as "B2B"
2.1 Product description/Product definition
products and not to end-users.
This EPD covers mechanical locks, latches and similar security
devices, including locking plates, to be used in buildings. The 2.5 Base materials/Ancillary materials
sample group used to calculate the LCA data for this ARGE Composition of product analysed for this EPD:
EPD includes sashlocks, multipoint locks and night latches.
The values given are for the product analysed for this EPD.
For certain products covered by this EPD the placing on the Ranges of values for other products covered by the validity
market in the European Union/European Free Trade scope analysis are shown in brackets.
Association (EU/EFTA) (with the exception of Switzerland) has Name Value Unit
to be compliant with Regulation (EU) No. 305/2011 (CPR).
Zamak (0% – 63,73%) 64 %
These products need a declaration of performance taking into
Steel (20,96% – 91,25%) 21 %
consideration EN 12209:2003, Building hardware – Locks and
latches – Mechanically operated locks, latches and locking Brass (3,31% – 9,21%) 9 %
plates – Requirements and test methods and the CE-marking. Nickel silver (0% – 5,49%) 6 %
Bronze (0% – 0,44%) 0 %
For the other products no legal provisions for harmonisation in
Zamak is an alloy with a base metal of zinc and alloying
the EU exist. They may be designed and manufactured
elements of aluminium, magnesium, and copper. Components
according to EN 12209:2016, Building hardware – Mechanically
made of Zamak are die-cast.
operated locks and locking plates – Requirements and test
methods or prEN 15685, Building hardware – Requirements
Steel is produced by combining iron with carbon as well as
and test methods – Multipoint locks, latches and locking plates
other elements depending on the desired characteristics.
– Characteristics and test methods.
Components made of steel are formed by stamping or other
types of mechanical processing.
For the application and use the respective national provisions
at the place of use apply.
Brass is an alloy of zinc and copper. Components made of
2.2 Application brass are made by extrusion, forging, die-casting or other types
These products are designed to be used in door, window and of mechanical processing.
shutter assemblies consisting of various materials and used for
various applications. Their purpose is to ensure the fastening of Nickel silver is an alloy of copper, nickel, and zinc.
doors, windows or shutters in the closed position. In respect of Components made of nickel silver are formed by stamping or
doors, they can be used on either interior or exterior doors. other types of mechanical processing.
2.3 Technical Data Bronze is an alloy consisting primarily of copper, commonly
Ideally, products should comply with a suitable technical with tin and often with the addition of other metals and
specification. EN 12209 and prEN 15685 are examples of such sometimes non-metals. Components can be bronze-coated for
a specification and some products will comply with them. The decorative reasons and for providing sliding and dry running
relevant grading structure according to EN 12209 is shown in properties.
the following table:
Name Value Unit 1) This product/article/at least one partial article contains
substances listed in the ECHA candidate list (date: 14.06.2023)
Category of use 1 - 3 Grade
exceeding 0.1 percentage by mass: Certain components may
Durability A,B,C,L,M,R,S,W,X Grade
contain small amounts of lead (CAS no. 7439-92-1) as an
Door mass and closing force 0 - 9 Grade
alloying element.
Suitability for use in fire resisting
0,A,B,N Grade
and/or smoke control door sets 2) This product/article/at least one partial article contains other
Safety 0 Grade cancerogenic, mutagenic, reprotoxic (CMR) substances in
Corrosion resistance 0,A,C,D,F,G Grade categories 1A or 1B which are not on the ECHA candidate list,
exceeding 0.1 percentage by mass: no.
Security - burglar resistance 0 - 7 Grade
Key identification of lever locks 0,A,B,C,D,E,F,G,H Grade
3) Biocide products were added to this construction product or it
The quoted standard defines the requirements of the product has been treated with biocide products (this then concerns a
and the associated test methods. As construction hardware treated product as defined by the (EU) Ordinance on Biocide
products are part of a set of a construction products (doorset, Products No. 528/2012): no.
window, shutter), European application standards for locks
2.6 Manufacture
themselves do not exist.
The manufacture of a lock usually follows a 3-step procedure:
If applicable, performance data of the product need to be in 1. Manufacture of the components: this step may include
accordance with the declaration of performance with respect to surface treatment in the factory or by external
its essential characteristics according to EN 12209:2003, contractors.
Building hardware - Mechanically operated locks and locking 2. Pre-assembly of modules (in the factory).
plates - Requirements and test methods. 3. Final assembly (in the factory).
2.4 Delivery status 2.7 Environment and health during manufacturing
The products are sold by unit. Deliveries of individual items are Regular measurements of air quality and noise levels are
possible but are an exception. Standard deliveries comprise a carried out by the manufacturers, the ARGE member
2 Environmental Product Declaration - ARGE – The European Federation of Locks and Building Hardware Manufacturers - Locks
companies. The results shall be within the mandatory safety of use and environmental conditions. It is required that
levels. In areas where employees are exposed to chemical installation as well as maintenance of the product are done in
products, the required protective clothing and technical line with instructions provided by the manufacturer.
protective devices shall be provided. Regular health checks are
mandatory for employees in production facilities. 2.13 Extraordinary effects
Fire
2.8 Product processing/Installation Certain products are suitable for use on fire resisting and/or
The installation of the product may vary depending on the type smoke control door/window sets according to one of the
of door, window or shutter and the specific situation, but the classes A,B,N in EN 12209.
products shall not require energy consumption for installation.
Water
2.9 Packaging The declared product is intended to be used in a building under
Normally, each individual product is packed in paper or normal conditions (indoor and outdoor use). It shall not emit
cardboard. These individual products are then packed in a hazardous substances in the event of flooding.
cardboard box and stacked on wooden pallets for transport to
the customer. Mechanical destruction
Mechanical destruction of the declared product shall not
Waste from product packaging is collected separately for waste materially alter its composition or have any adverse effect on
disposal (including recycling). the environment.
2.10 Condition of use 2.14 Re-use phase
Once installed, the products shall require no servicing during Removal of locks (for re-use or recycling) shall have no adverse
their expected service lives. There shall be no consumption of effect on the environment.
water or energy linked to their use, and they shall not cause
any emissions. 2.15 Disposal
Locks should be recycled wherever possible, providing that
2.11 Environment and health during use there is no adverse effect on the environment. The waste code
No environmental damage or health risks are to be expected in accordance with the European Waste Code is 17 04 07.
during normal conditions of use.
2.16 Further information
2.12 Reference service life
Details of all types and variants can be found on the
The reference service life is 30 years under normal working manufacturers' websites. The respective website addresses are
conditions. This corresponds to passing a mechanical available at https://arge.org.
endurance test of 100.000 cycles as specified in EN 12209.
The reference service life is dependent on the actual frequency
3. LCA: Calculation rules
There is no waste associated with the installation of the
3.1 Declared Unit product. The A5 module therefore represents only the disposal
The declared unit for all products covered by ARGE EPD is 1 of the product packaging.
kg (of product). Since individual products will rarely weigh The End-of-Life (EoL) stages are also considered. The
exactly 1 kg it is necessary to establish the exact weight of the transportation to the EoL disposal site is taken into account in
product and then use this as a correction factor to determine module C2. Module C4 covers the disposal of the locks. Module
the true values for 1 kg of product in the tables (Section 5). C3 covers the recycling of the individual elements according to
Declared unit European averages, with the remaining waste divided between
incineration and landfill. Such a mixed scenario is declared due
Name Value Unit
to the complex material mix of the product and the dependency
Declared unit 1 kg
of the EoL-route on the EoL route of the product the lock has
Mass of declared Product 1.64 kg been integrated into.
Raw density 1 kg/m3 In practice, the end of life has been modelled as follows:
• when a material is sent for recycling, generic transport
and electric consumption of a shredder is taken into
3.2 System boundary account (corresponding to the process 'Grinding,
Type of the EPD: "cradle to gate with options, with modules C1 metals'). Only then, is the material considered to have
– C4, and module D (A1-A3, C1-C3, D and additional attained the 'end-of-waste' state.
modules)" • each type of waste is modelled as a transport to the
treatment site with a distance of 30 km. Parts sent for
The analysis of the product life cycle includes the production recycling include electricity consumption (grinding) and
and transport of the raw materials, the manufacture of the a flow ('Materials for recycling, unspecified').
product and the packaging materials which are declared in
3.3 Estimates and assumptions
modules A1-A3.
Losses during production are considered as waste and are sent The LCA data of the declared lock have been calculated using
for recycling. No recycling processes are taken into account the production data of 9 ARGE member companies. These
except for transport and electricity consumption for grinding the companies have been chosen by ARGE as being
metals. When recycled metals are used as raw material only representative of their production processes and their market
their transformation process is taken into account and not the shares. The lock chosen as representative for this calculation
extraction of the raw material. follows the "worst-case" principle as explained under 6. LCA
interpretation.
A4 module represents the transport of the finished locks to the
installation site.
3 Environmental Product Declaration - ARGE – The European Federation of Locks and Building Hardware Manufacturers - Locks
Geography: Data come from production sites of the ARGE
3.4 Cut-off criteria member companies. Generic data come from the ecoinvent
The cut-off criteria considered are 1% of renewable and non- database, representative for European production processes.
renewable primary energy usage and 1% of the total mass of
that unit process. The total neglected input flows per module Technology: Material shaping technologies are based on
amount to a maximum of 5% of energy usage and mass. European technology in the case of the use of generic data.
For this study, all input and output flows have been considered A total of 8 typical products (based on sales figures) have been
at 100%, including raw materials as per the product evaluated, and the worst-case results are used in the tables.
composition provided by the manufacturer and packaging of
raw materials as well as the final product. Energy and water 3.7 Period under review
consumptions have also been considered at 100% according to The data of the LCA is based on the annual production data of
the data provided. an ARGE member from 2013, considered representative for the
year 2022.
With the approach chosen, no significant environmental
impacts are known to have been cut off. 3.8 Geographic Representativeness
Land or region, in which the declared product system is
3.5 Background data manufactured, used or handled at the end of the product´s
For the life cycle modelling of the considered product, all lifespan: Europe
relevant background datasets are taken from ecoinvent v3.8
(system model: cut-off by classification).
3.9 Allocation
3.6 Data quality The products are produced in numerous production sites. All
The objective of this evaluation is to evaluate the environmental data were provided by the manufacturers of the products per
impacts generated by the products throughout their entire life unit, and then divided by the mass of the product to give a
cycles. To this end, ISO 14040, ISO 14044 and EN 15804 have value per kg of product produced.
been met regarding the quality of data on the following different
criteria: The assumptions relating to the EoL of the product and waste
during its life cycle are described in the section System
Time: The life cycle inventory data used come from: Boundaries. Metal losses during production (stage A3) are
considered as waste.
• Data collected specifically for this study on the ARGE
member companies' manufacturing sites. Datasets are
3.10 Comparability
based on 1-year averaged data (time period: January
Basically, a comparison or an evaluation of EPD data is only
2013 to December 2013 considered representative for
possible if all the data sets to be compared were created
2022).
according to EN 15804 and the building context, respectively
• In the absence of collected data, generic data from the
the product-specific characteristics of performance, are taken
ecoinvent v3.8 database have been used. This is
into account.
updated regularly and is representative of current
processes (the entire database having been updated in
ecoinvent v3.8 (system model: cut-off by classification) has
2021).
been used as the background database.
4. LCA: Scenarios and additional technical information
Name Value Unit
Characteristic product properties of biogenic carbon
Material loss - kg
Output substances following waste treatment on
Information on biogenic carbon content at factory gate site 0.135 kg
Note: 1 kg of biogenic carbon is equivalent to 44/12 kg of CO 2.
Reference service life
Name Value Unit
Name Value Unit
kg
Biogenic carbon content in product 0 C Reference service life 30 a
Biogenic carbon content in accompanying kg Test cycles over RSL (EN 12209) 100'000 cycles
0.055
packaging C
End of life (C1-C4)
Name Value Unit
The following information is the basis of the declared modules
Collected separately waste type 1 kg
within the LCA in this EPD.
Recycling 0.281 kg
Transport to the building site (A4)
Energy recovery 0.331 kg
Name Value Unit
Landfilling 0.388 kg
Litres of fuel 25.8 l/100km
It is assumed that a 16–32-ton truck is used to transport the
Transport distance 3500 km
product:
Capacity utilisation (including empty runs) 36 %
- Transport to shredding facility for metal recovery: 150 km
- Transport to municipal waste incineration plant: 50 km
Installation into the building (A5)
- Transport to landfill: 30 km
Reuse, recovery and/or recycling potentials (D), relevant
scenario information
4 Environmental Product Declaration - ARGE – The European Federation of Locks and Building Hardware Manufacturers - Locks
Module D contains the benefits and loads beyond the system - net amounts of a metal leaving the product system are
boundary related to the recycling of metals, which result from quantified as the material for recycling leaving modules A1-C4
the treatment of recycled materials from the point of end-of- minus the input of secondary scrap (secondary material, SM) to
waste status to the point of substitution (as costs) and the the product system;
substitution of primary resources (as benefits). - in the case of brass and zinc alloys, which are composed of
two different constituting metals, no difference shall be made
According to EN 16710, clause 6.4.3.3: 'In module D between the input of secondary constituting metals (Cu and Zn;
substitution effects are calculated only for the resulting net Cu and Sn) and its alloys (CuZn; CuSn).
output flow.
Negative net output flows have been considered in the
For building hardware, the following rules apply for the quantification of module D.
quantification of net output flows:
- all production scrap and cuttings leave modules A1-B3 as It also includes the benefits and loads related to 'exported
sorted scrap without allocated burdens from primary production; energy electricity' and 'exported energy heat' resulting from the
the corresponding amounts are declared as material for energy recovery from plastic wastes in a municipal waste
recycling (MFR); incineration plant as modelled in Modules A3, A5 and C4.
5 Environmental Product Declaration - ARGE – The European Federation of Locks and Building Hardware Manufacturers - Locks
5. LCA: Results
In Table 1 "Description of the system boundary", the declared modules are indicated with an "X"; all modules that are not declared
within the EPD but where additional data are available are indicated with "MND". Those data can also be used for building assessment
scenarios. The values are declared with three valid digits in exponential form.
The set of characterisation factors EF3.0 has been used for the life cycle assessment.
DESCRIPTION OF THE SYSTEM BOUNDARY (X = INCLUDED IN LCA; MND = MODULE OR INDICATOR NOT DECLARED; MNR
= MODULE NOT RELEVANT)
Benefits and
Construction loads beyond
Product stage Use stage End of life stage
process stage the system
boundaries
la ire wta am R y lp p u s tro p s n a rT g n iru tc a fu n a M tro p s nm ae o rh r
T
f te tis e h t o t e ta g y lb m e s s A e s U e c n a n e tn ia M ria p e R tn e m e c a lp e R tn e m h s ib ru fe R la n o ity ag rr ee pn Oe e s u la n o ita r re et pa Ow e s u n o itc u rts n eo Dc -n o itilo m e d tro p s n a rT g n is s ee tsc ao Wrp la s o p s iD e s u e R- y re v o c e R- g n ilc y c e R- la itn e to p
A1 A2 A3 A4 A5 B1 B2 B3 B4 B5 B6 B7 C1 C2 C3 C4 D
X X X X X MND MND MNR MNR MNR MND MND X X X X X
RESULTS OF THE LCA - ENVIRONMENTAL IMPACT according to EN 15804+A2: 1 kg of locks
Parameter Unit A1-A3 A4 A5 C1 C2 C3 C4 D
GWP-total kg CO2 eq 5.62E+00 6.47E-01 2.06E-01 0 1.51E-02 3.16E-03 1.1E-02 -2.02E+00
GWP-fossil kg CO2 eq 5.81E+00 6.47E-01 2.94E-03 0 1.51E-02 3.15E-03 1.1E-02 -2.01E+00
GWP-biogenic kg CO2 eq -2.03E-01 0 2.03E-01 0 0 0 0 0
GWP-luluc kg CO2 eq 1.48E-02 2.59E-04 9.01E-07 0 6.02E-06 7.85E-06 3.49E-06 -5.56E-03
ODP kg CFC11 eq 3.55E-07 1.5E-07 4.59E-10 0 3.49E-09 1.6E-10 1.21E-09 -8.36E-08
AP mol H+ eq 1.32E-01 1.84E-03 2.15E-05 0 4.28E-05 1.62E-05 3.12E-05 -5.21E-02
EP-freshwater kg P eq 6.38E-04 4.61E-06 3.24E-08 0 1.07E-07 3.54E-07 6.72E-08 -1.94E-04
EP-marine kg N eq 9.62E-03 3.65E-04 9.22E-06 0 8.5E-06 2.08E-06 1.09E-05 -2.92E-03
EP-terrestrial mol N eq 1.17E-01 4.07E-03 9.85E-05 0 9.47E-05 2.4E-05 1.16E-04 -3.6E-02
kg NMVOC
POCP 3.46E-02 1.56E-03 2.54E-05 0 3.64E-05 6.57E-06 3.52E-05 -1.14E-02
eq
ADPE kg Sb eq 2.62E-03 2.29E-06 8.64E-09 0 5.34E-08 7.63E-09 1.39E-08 -1.21E-03
ADPF MJ 6.67E+01 9.81E+00 3.42E-02 0 2.28E-01 6.67E-02 8.87E-02 -2.16E+01
m3 world eq
WDP 3.14E+00 2.99E-02 3.34E-04 0 6.95E-04 7.45E-04 -9.63E-04 -8.41E-01
deprived
GWP = Global warming potential; ODP = Depletion potential of the stratospheric ozone layer; AP = Acidification potential of land and water; EP =
Eutrophication potential; POCP = Formation potential of tropospheric ozone photochemical oxidants; ADPE = Abiotic depletion potential for non-fossil
resources; ADPF = Abiotic depletion potential for fossil resources; WDP = Water (user) deprivation potential)
RESULTS OF THE LCA - INDICATORS TO DESCRIBE RESOURCE USE according to EN 15804+A2: 1 kg of locks
Parameter Unit A1-A3 A4 A5 C1 C2 C3 C4 D
PERE MJ 1.15E+01 1.38E-01 -1.76E+00 0 3.21E-03 1.27E-02 1.4E-03 -3.04E+00
PERM MJ 2.54E+00 0 1.37E+00 0 0 0 0 0
PERT MJ 1.4E+01 1.38E-01 -3.93E-01 0 3.21E-03 1.27E-02 1.4E-03 -3.04E+00
PENRE MJ 6.67E+01 9.81E+00 3.42E-02 0 2.28E-01 6.73E-02 1.71E-01 -2.17E+01
PENRM MJ 1.62E-01 0 0 0 0 0 -8.21E-02 0
PENRT MJ 6.68E+01 9.81E+00 3.42E-02 0 2.28E-01 6.73E-02 8.87E-02 -2.17E+01
SM kg 1.08E-01 0 0 0 0 0 0 0
RSF MJ 0 0 0 0 0 0 0 0
NRSF MJ 0 0 0 0 0 0 0 0
FW m3 8.58E-02 1.04E-03 8.72E-05 0 2.42E-05 4.3E-05 2.17E-04 -2.35E-02
PERE = Use of renewable primary energy excluding renewable primary energy resources used as raw materials; PERM = Use of renewable primary
energy resources used as raw materials; PERT = Total use of renewable primary energy resources; PENRE = Use of non-renewable primary energy
excluding non-renewable primary energy resources used as raw materials; PENRM = Use of non-renewable primary energy resources used as raw
materials; PENRT = Total use of non-renewable primary energy resources; SM = Use of secondary material; RSF = Use of renewable secondary fuels;
NRSF = Use of non-renewable secondary fuels; FW = Use of net fresh water
RESULTS OF THE LCA – WASTE CATEGORIES AND OUTPUT FLOWS according to EN 15804+A2:
1 kg of locks
Parameter Unit A1-A3 A4 A5 C1 C2 C3 C4 D
HWD kg 4.69E-04 2.56E-05 2.77E-07 0 5.96E-07 2.37E-08 1.71E-07 -1.57E-04
NHWD kg 1.99E+00 5.16E-01 2.91E-03 0 1.2E-02 2.51E-04 3.8E-01 -3.71E-01
RWD kg 3.67E-04 1.42E-04 3.76E-07 0 3.3E-06 8.97E-07 1.14E-06 -7.97E-05
CRU kg 0 0 0 0 0 0 0 0
MFR kg 1.11E-01 0 2.38E-02 0 0 4.71E-01 0 0
MER kg 0 0 0 0 0 0 0 0
6 Environmental Product Declaration - ARGE – The European Federation of Locks and Building Hardware Manufacturers - Locks
EEE MJ 6.97E-04 0 6.16E-02 0 0 0 3.48E-03 0
EET MJ 4.62E-03 0 4.08E-01 0 0 0 2.3E-02 0
HWD = Hazardous waste disposed; NHWD = Non-hazardous waste disposed; RWD = Radioactive waste disposed; CRU = Components for re-use;
MFR = Materials for recycling; MER = Materials for energy recovery; EEE = Exported electrical energy; EET = Exported thermal energy
RESULTS OF THE LCA – additional impact categories according to EN 15804+A2-optional:
1 kg of locks
Parameter Unit A1-A3 A4 A5 C1 C2 C3 C4 D
Disease
PM 5.57E-07 5.2E-08 3.02E-10 0 1.21E-09 4.33E-11 9.37E-10 -1.76E-07
incidence
IR kBq U235 eq 1.96E-01 4.26E-02 1.18E-04 0 9.91E-04 6.07E-04 3.41E-04 -4.74E-02
ETP-fw CTUe 9.36E+02 7.7E+00 3.96E-02 0 1.79E-01 3.36E-02 2.12E-01 -3.15E+02
HTP-c CTUh 3.53E-08 2.48E-10 4.66E-12 0 5.76E-12 8.97E-13 9.85E-12 -1.12E-08
HTP-nc CTUh 1.7E-06 7.78E-09 2.12E-10 0 1.81E-10 2.91E-11 9.49E-11 -6.54E-07
SQP SQP 7.05E+01 6.84E+00 1.91E-02 0 1.59E-01 1.03E-02 1.51E-01 -1.66E+01
PM = Potential incidence of disease due to PM emissions; IR = Potential Human exposure efficiency relative to U235; ETP-fw = Potential comparative
Toxic Unit for ecosystems; HTP-c = Potential comparative Toxic Unit for humans (cancerogenic); HTP-nc = Potential comparative Toxic Unit for humans
(not cancerogenic); SQP = Potential soil quality index
Disclaimer 1 – for the indicator 'Potential Human exposure efficiency relative to U235'. This impact category deals mainly with the
eventual impact of low-dose ionizing radiation on human health of the nuclear fuel cycle. It does not consider effects due to possible
nuclear accidents, occupational exposure or radioactive waste disposal in underground facilities. Potential ionizing radiation from the
soil, radon and from some construction materials is also not measured by this indicator.
Disclaimer 2 – for the indicators 'abiotic depletion potential for non-fossil resources', 'abiotic depletion potential for fossil resources',
'water (user) deprivation potential, deprivation-weighted water consumption', 'potential comparative toxic unit for ecosystems', 'potential
comparative toxic unit for humans – cancerogenic', 'Potential comparative toxic unit for humans - not cancerogenic', 'potential soil
quality index'. The results of this environmental impact indicator shall be used with care as the uncertainties on these results are high
as there is limited experience with the indicator.
6. LCA: Interpretation
7 Environmental Product Declaration - ARGE – The European Federation of Locks and Building Hardware Manufacturers - Locks
The following figure illustrates the relative contributions of the different modules along the life cycle of the declared products:
Figure 1: Environmental impacts of locks along its life Benefits and burdens beyond the system boundary (module D)
cycle (impacts from production modules A1-A3 = 100 %) are in the order of 15 % to 30 % of the impacts over the product
life cycle (modules A1-A3) and relate basically to the recycling
The largest part of environmental impacts is caused during of metals.
production (modules A1-A3); comparably small impacts are
caused during the transport of the product to the construction A total of 9 typical products (based on sales figures) have been
site (via the manufacturer of the product, which the lock has evaluated and the worst-case results are used in section 5 of
been integrated into). this EPD. In chapter 2.5, the tabulated range of relative weight
per material ensures that the variability of results stays within
All the other modules related to the product life cycle are not +/- 40% of the declared values (assessed for the indicators
significant. GWP, PENRT, and non-hazardous waste).
7. Requisite evidence
No testing results are required by the PCR part B.
8. References
Product category rules of IBU EN 17610:2022, Building hardware - Environmental product
declarations - Product category rules complementary to EN
IBU (2021) 15804 for building hardware.
IBU (2021): General Instructions for the EPD Programme of the
Institut Bauen und Umwelt e.V. (General Instructions for the ISO 14025
IBU EPD Programme). Version 2.0, Institut Bauen und Umwelt, ISO 14025:2006-07, Environmental labels and declarations -
Berlin. Type III Environmental declarations - Principles and
procedures.
IBU (2021)
IBU (2021): PCR Part A: Calculation rules for the life cycle ISO 14044
assessment and requirements on the project report according EN ISO 14044:2006-07, Environmental management - Life
to EN 15804+A2. Version 1.3., Institut Bauen und Umwelt, cycle assessment - Requirements and guidance (ISO
Berlin. 14044:2006).
IBU (2023) EN 12209
IBU (2023): PCR Part B: Requirements on the EPD for building EN 12209:2003, Building hardware – Locks and latches –
hardware products, Institut Bauen und Umwelt, Berlin. Mechanically operated locks, latches and locking plates –
Requirements and test methods. (harmonised)
Standards and legal documents EN 12209:2016, Building hardware – Mechanically operated
locks and locking plates – Requirements and test methods. (not
EN 15804 harmonised)
EN 15804:2012+A2:2019+AC:2021, Sustainability of
construction works - Environmental product declarations - Core prEN 15685
rules for the product category construction products. prEN 15685:2022, Building hardware – Requirements and test
methods – Multipoint locks, latches and locking plates –
EN 17610 Characteristics and test methods.
8 Environmental Product Declaration - ARGE – The European Federation of Locks and Building Hardware Manufacturers - Locks
PARLIAMENT AND OF THE COUNCIL of 22 May 2012
EN 13501-1 concerning the making available on the market and use of
EN 13501-1:2018, Fire classification of construction products biocidal products.
and building elements - Part 1: Classification using data from
reaction to fire tests. European List of Waste
Commission Decision of 3 May 2000 replacing Decision
ISO 15686 94/3/EC establishing a list of wastes pursuant to Article 1(a) of
ISO 15686:1, -2, -7 and -8. Service life planning (various parts). Council Directive 75/442/EEC on waste and Council Decision
94/904/EC establishing a list of hazardous waste pursuant to
Regulation No. 305/2011 Article 1(4) of Council Directive 91/689/EEC on hazardous
Regulation No. 305/2011 (Construction Products Regulation, or waste (notified under document number C(2000) 1147).
CPR) of the European Parliament and of the European Council
is a regulation of 9 March 2011 that lays down harmonised Additional references
conditions for the marketing of construction products and
replaces Construction Products Directive (89/106/EEC). BBSR 2017
BBSR (2017): Nutzungsdauer von Bauteilen in
ECHA candidate list Lebenszyklusanalysen nach Bewertungssystem Nachhaltiges
Candidate List of substances of very high concern for Bauen (BNB). Version vom 24.10.2017, Bundesinstitut für Bau-,
Authorisation, published in accordance with Article 59(10) of the Stadt- und Raumforschung, Berlin.
REACH Regulation. European Chemicals Agency, Brussels.
ecoinvent v3.8
Ordinance on Biocide Products No. 528/2012 http://www.ecoinvent.org
REGULATION (EU) No 528/2012 OF THE EUROPEAN
9 Environmental Product Declaration - ARGE – The European Federation of Locks and Building Hardware Manufacturers - Locks
Publisher
Institut Bauen und Umwelt e.V. +49 (0)30 3087748- 0
Hegelplatz 1 info@ibu-epd.com
10117 Berlin www.ibu-epd.com
Germany
Programme holder
Institut Bauen und Umwelt e.V. +49 (0)30 3087748- 0
Hegelplatz 1 info@ibu-epd.com
10117 Berlin www.ibu-epd.com
Germany
Author of the Life Cycle Assessment
Dr. Frank Werner - Umwelt & Entwicklung + 41 (0)44 241 39 06
Kammelenbergstrasse 30 frank@frankwerner.ch
9011 St. Gallen http://www.frankwerner.ch/
Switzerland
Owner of the Declaration
ARGE – The European Federation of Locks and +49 (0)2051 9506 15
Building Hardware Manufacturers mail@arge.org
Offerstraße 12 www.arge.org
42551 Velbert
Germany
10 Environmental Product Declaration - ARGE – The European Federation of Locks and Building Hardware Manufacturers - Locks
