ENVIRONMENTAL PRODUCT DECLARATION
as per ISO 14025 and EN 15804+A2
Owner of the Declaration Schüco International KG
Publisher Institut Bauen und Umwelt e.V. (IBU)
Programme holder Institut Bauen und Umwelt e.V. (IBU)
Declaration number EPD-SCH-20230390-CBA1-EN
Issue date 23.10.2023
Valid to 22.10.2028
Schüco Aluminium Profile
Schüco International KG
www.ibu-epd.com | https://epd-online.com
General Information
Schüco International KG Schüco Aluminium Profile
Programme holder Owner of the declaration
IBU – Institut Bauen und Umwelt e.V. Schüco International KG
Hegelplatz 1 Karolinenstraße 1-15
10117 Berlin 33609 Bielefeld
Germany Germany
Declaration number Declared product / declared unit
EPD-SCH-20230390-CBA1-EN 1 kg plate finish, Schüco aluminium profile
This declaration is based on the product category rules: Scope:
Products of aluminium and aluminium alloys, 01.08.2021 The present environmental product declaration concerns the 1 kg plate
(PCR checked and approved by the SVR) finished Schüco aluminium profile.
This EPD is based on data from aluminium pressing plants which produce
Issue date aluminium profiles with comparable environmental attributes. The creation
of these aluminium profiles requires technically similar production
23.10.2023
processes. In this EPD, the aluminium used in the extrusion process refers
to the production of primary aluminium in Europe.
Valid to
The data collected for this EPD refers to 2022.
22.10.2028
The owner of the declaration shall be liable for the underlying information
and evidence; the IBU shall not be liable with respect to manufacturer
information, life cycle assessment data and evidences.
The EPD was created according to the specifications of EN 15804+A2. In
the following, the standard will be simplified as EN 15804.
Verification
The standard EN 15804 serves as the core PCR
Independent verification of the declaration and data according to ISO
14025:2011
Dipl.-Ing. Hans Peters
(Chairman of Institut Bauen und Umwelt e.V.) internally X externally
Florian Pronold Matthias Schulz,
(Managing Director Institut Bauen und Umwelt e.V.) (Independent verifier)
1 Environmental Product Declaration - Schüco International KG - Schüco Aluminium Profile
Product
Constructional data
Product description/Product definition
The aluminium profiles produced are semi-finished products for Name Value Unit
use in Schüco windows, doors and façade systems. Gross density 2700 kg/m3
Melting point 660 °C
The Schüco aluminium profiles are made out of aluminium
Thermal conductivity 200 W/(mK)
alloys consisting of light metal aluminium (Al) and various
alloying elements (such as silicon, copper, manganese,
Modulus of elasticity 70000 N/mm2
magnesium etc.). The aluminium used in the extrusion process Shear modulus 27000 N/mm2
refers to the production of primary aluminium in Europe. Specific heat capacity 0.9 kJ/kgK
Hardness 65 HB
The raw aluminium profiles can be anodised, wet or powder-
Yield strength Rp 0,2 min. 160 N/mm2
coated (as required by the customer).
Tensile strength Rm min. 200 N/mm2
Relevant standards Tensile stress at break 8 %
Whether aluminium profiles are subject to harmonisation
Construction data (as in PCR B: Requirements on the EPD for
regulations or not depends on whether these carry a load in the
Products of aluminum and aluminum alloys listed, e.g. electrical
final application (e.g. window frames or support beams).
conductivity, coefficient of thermal expansion and the chemical
However, since the aluminium profiles are intermediate
composition) are not relevant for this product.
products, it is not possible to make a clear statement about
their final application. For this reason, both standards ("Profiles
Profiles and constructions in accordance with CPR (hEN):
and constructions in accordance with CPR" and "Profiles that
Performance values of the product corresponding to the
are not subject to the EU harmonisation regulations") are listed
Declaration of Performance in relation to its essential features
below in order to cover the scope of the possible end uses of
as per:
the aluminium profiles.
• EN 15088, Aluminium and aluminium alloys – Structural
Profiles and constructions in accordance with CPR (hEN): The products for construction works –Technical conditions
regulation (EU) No. 305/2011 (CPR) applies to bringing the for inspection and delivery
product into circulation in the European Union/European Free • EN 1090-3, Execution of steel structures and aluminium
Trade Association (EU/EFTA) (with the exception of structures - Part 3: Technical requirements for
Switzerland). The product requires a Declaration of aluminium structures
Performance taking into account the following standards:
Profiles that are not subject to any EU harmonisation
• EN 15088, Aluminium and aluminium alloys – Structural
legislation: Performance values of the product in regard to its
products for construction works –Technical conditions
features in accordance with the controlled technical regulations
for inspection and delivery
(no CE marking).
• EN 1090-3, Execution of steel structures and aluminium
structures - Part 3: Technical requirements for
Delivery condition
aluminium structures
Materials delivered in accordance with EN 755-1 or
EN 12020-1. The alloys comply with EN 573-3 regarding their
With regard to use, the respective national regulations apply.
chemical composition. The aluminium profiles are packaged in
accordance with customer requirements.
Profiles that are not subject to any EU harmonisation
legislation:
Base materials/Ancillary materials
With regard to using the product, the respective national
The chemical composition of aluminum alloys of the 6000
regulations apply for the location of application
series - AlMgSi (specifically EN AW-6060/6063; EN AW-6005)
• EN 755-1, Aluminium and aluminium alloys – Extruded can be found in standard EN 573-3 (limit values for alloying
rod/bar, tube and profiles –Part 1: Technical conditions elements). The aluminum content is > 90%. The other alloy
for inspection and delivery components are magnesium, silicon, iron, copper, manganese,
• EN 12020-1, Aluminium and aluminium alloys - chromium, zinc, titanium.
Extruded precision profiles in alloys EN AW-6060 and
EN AW-6063 - Part 1: Technical conditions for Material note: Aluminium is a light metal. The melting point of
inspection and delivery pure aluminium is 660 °C. The natural colour is silvery-white.
Application
Aluminium is very corrosion-resistant and has a long service
Aluminium profiles are used in Schüco windows, doors and life. A naturally thin oxide layer protects the material from
façade systems. degradation due to air, water or certain chemicals.
Technical Data
The properties make it possible to manufacture profiles with
Physical properties of aluminum (e.g. EN AW-6060/6063; EN
complex shapes.
AW-6005):
This product/article/at least one partial article contains
substances listed in the candidate list (date: 28.09.2023)
exceeding 0.1 percentage by mass: no.
This product/article/at least one partial article contains other
CMR substances in categories 1A or 1B which are not on the
2 Environmental Product Declaration - Schüco International KG - Schüco Aluminium Profile
candidate list, exceeding 0.1 percentage by mass: no. comply with the semi-finished products created but instead are
specific to the design and the intended application of the end
Biocide products were added to this construction product or it product.
has been treated with biocide products (this then concerns a
treated product as defined by the (EU) Ordinance on Biocide Reference service life
Products No. 528/2012): no. An expected life cycle is not declared for aluminium profiles as
these are semi-finished products. The service life is dependent
Manufacture on the product application. As aluminium is protected by an
Cutting – The aluminium billets are cut to size. oxide layer on the surface itself, the service life is, in theory,
unlimited.
Heating – The aluminium billets are heated in an oven to
between 460 °C and 530 °C so that it is easier to reach the Exceptional fire effects
plastic state of the metal during shaping. In accordance with DIN 4102-4, uncoated aluminium profiles
fulfil the requirements of building material class A, "non-
Extrusion – With typical compression of 6000–8000 MN/mm² on flammable". The melting point of the aluminium material is 660
a cross-sectional area of the billet, the hot aluminium billet is °C.
pressed through a pre-heated die. This is how the profile gets • Smoke gas development: No smoke gas develops with
its geometric shape. the profiles.
• Burning drops of liquid: Not applicable
Chilling – The profiles are cooled directly after the extrusion • Toxicity of combustion gases: Not applicable
(there are various processes that use air, water or spray). The
cooling is necessary to achieve the final strength. Water
The exposure of the profiles to water does not lead to any
Elongation – After extrusion the profiles are elongated in order changes in the product nor to any negative consequences for
to straighten them out. Cutting to length – Cutting the profiles the environment.
according to customer requirements (default 6000 mm).
Mechanical destruction
Tempering – Hardening of the profiles at a temperature Mechanical destruction is not relevant for aluminium profiles.
between 145 °C and 210 °C (5–12 hours).
Period of post use
Packaging – This is followed by packing the profiles in Aluminium profiles are fully recyclable. The material does not
accordance with customer requirements. suffer any loss in quality from this process. Scrap from
demolitions, conversions or renovations can be easily
Environment and health & safety during manufacture separated and (via the recycling industry) fed into the recycling
Throughout the entire manufacturing process, all legal process.
obligations regarding occupational health and safety and the
environment are fulfilled. All of the process scrap that occurs during the manufacture and
further processing of the profile in the factory is collected and
Production fabrication/installation processed into new primary material (billets, bars, ...) in a
Throughout the entire manufacturing process, all legal recycling process in the remelting plant. These billets are then
obligations regarding occupational health and safety and the used in the plant as a new starting material.
environment are fulfilled.
Disposal
Packaging In accordance with the European Waste Catalogue (EWC) the
All profiles are individually packaged in accordance with end product complies with the disposal code (170402
customer requirements. The packing materials used range from Aluminium).
reusable containers, untreated wooden crates and pallets to
cardboard packaging etc. Due to its high value as a raw material, aluminium scrap is not
disposed of. Instead, it is fed into an established circle of reuse
In order to protect the profiles, they are packaged separately or recycling.
with cardboard intermediate layers, polyethylene (PE) foil and
paper, for example. The PE foil, paper and cardboard used can
be fed into the recycling process by the customer.
Condition during use
The profiles are made of an alloy which consists of aluminium
and the named alloying components. The constituents
correspond to the raw materials named in EN 573-3 with the
specified mass percentage shares.
There are no special features of the material composition for
the period of use.
Environment and health & safety during use
The intended use of the aluminium profiles does not pose any
risks to water, air/the atmosphere or soil.
The specifications regarding use and maintenance do not
3 Environmental Product Declaration - Schüco International KG - Schüco Aluminium Profile
LCA: Calculation rules
Declared Unit Module C2 includes transportation of post-consumer waste to
The declared unit refers to 1 kg of extruded aluminium profile. waste processing.
Declared unit and mass reference
Module C3 does not include environmental impacts, as
Name Value Unit
aluminium waste reaches its end-of-waste status after
Declared unit 1 kg
dismantling.
Geographically, the study represents the production of
aluminium extrusion profiles in Central Europe. The background Module C4 does not include environmental impacts, as all 100
data for aluminium refers to European production of primary % of the waste is expected to be recycled.
aluminium.
Module D includes potential benefits from all net flows given in
System boundary modules A5 and C3 that leave the system boundary of the
Cradle to gate with options: modules A1–A3, C, D and product system after having past end-of-waste state in the form
additional modules A4 and A5 of recovery and/or recycling potentials.
Modules A1 to A3 include the supply of all materials, auxiliaries, Geographic Representativeness
energy and packaging materials up to the factory gate, as well Land or region, in which the declared product system is
as waste processing up to the end-of-waste state or disposal of manufactured, used or handled at the end of the product´s
final residues. Aluminium billets, produced from remelted lifespan: Europe
production scrap, stay within the product system and are
reused within A3.
Comparability
Basically, a comparison or an evaluation of EPD data is only
Module A4 includes transport of the aluminium profile to the
possible if all the data sets to be compared were created
place of installation or further processing.
according to EN 15804 and the building context, respectively
the product-specific characteristics of performance, are taken
Module A5 includes the disposal of packaging material.
into account. LCAfE software and MLC databases (f.k.a. GaBi)
by Sphera Solutions GmbH were used for all background
Module C1 includes the energy demand for dismantling and
databases and LCA calculations.
separation of materials.
LCA: Scenarios and additional technical information
End of Life (C1-C4)
Characteristic product properties of biogenic carbon
For dismantling and separation of built-in aluminium profiles at
The product itself does not contain any biogenic Carbon.
the end of life, the use of diesel-powered construction
Packaging material contain biogenic carbon from the use of
machinery is assumed in module C1.
wood and cardboard/ paper.
Name Value Unit
Note: 1 kg of biogenic carbon is equivalent to 44/12 kg of CO 2. Diesel used in construction machines (C1) 0.0056 kg
Information on biogenic carbon content at factory gate Transport distance in module C2 is considered with the listed
Name ValueUnit scenario settings.
kg Name Value Unit
Biogenic carbon content in product -
C Litres of fuel (C2) 0.0029 l/100km
Biogenic carbon content in accompanying kg Transport distance (C2) 50 km
0.021
packaging C Capacity utilisation (including empty runs) 61 %
The following technical information is a basis for the declared
modules or can be used for developing specific scenarios in the Collection rate of aluminium scrap at the end of life is set to 100
context of a building assessment. %.
Name Value Unit
Transport to the building site (A4) Collected separately waste type (aluminium) 1 kg
Name Value Unit
Reuse, recovery and/or recycling potentials (D), relevant
Litres of fuel (A4) 0.0029 l/100km
scenario information
Transport distance (A4) 100 km
Recycling potentials are calculated for the amount of the net
Capacity utilisation (including empty runs) 61 %
flow aluminium scrap.
Installation into the building (A5) Name Value Unit
Name ValueUnit Net flow aluminium scrap 1 kg
Output substances following waste treatment on
0.056 kg
site packaging waste
4 Environmental Product Declaration - Schüco International KG - Schüco Aluminium Profile
LCA: Results
DESCRIPTION OF THE SYSTEM BOUNDARY (X = INCLUDED IN LCA; MND = MODULE OR INDICATOR NOT DECLARED; MNR
= MODULE NOT RELEVANT)
Benefits and
Construction loads beyond
Product stage Use stage End of life stage
process stage the system
boundaries
la ire ta m w a Ry lp p u s tro p s n a rT g n iru tc a fu n a M e h t m o rf tro p s n a rTe tis e h t o t e ta g y lb m e s s A e s U e c n a n e tn ia M ria p e R tn e m e c a lp e R tn e m h s ib ru fe R y g re n e la n o ita re p Oe s u re ta w la n o ita re p Oe s u n o itc u rts n o c -e Dn o itilo m e d tro p s n a rT g n is s e c o rp e ts a W la s o p s iD -e s u e R-y re v o c e R-g n ilc y c e Rla itn e to p
A1 A2 A3 A4 A5 B1 B2 B3 B4 B5 B6 B7 C1 C2 C3 C4 D
X X X X X MND MND MNR MNR MNR MND MND X X X X X
RESULTS OF THE LCA - ENVIRONMENTAL IMPACT according to EN 15804+A2: 1 kg Schüco Aluminium Profile
Parameter Unit A1-A3 A4 A5 C1 C2 C3 C4 D
GWP-total kg CO 2 eq 7.11E+00 8.69E-03 9.78E-02 1.99E-02 4.34E-03 0 0 -6.32E+00
GWP-fossil kg CO 2 eq 7.15E+00 8.58E-03 2.22E-02 1.96E-02 4.29E-03 0 0 -6.3E+00
GWP-biogenic kg CO 2 eq -4.49E-02 2.54E-05 7.57E-02 7.73E-05 1.27E-05 0 0 -2.03E-02
GWP-luluc kg CO 2 eq 1.83E-03 7.96E-05 3.61E-07 1.81E-04 3.98E-05 0 0 -1.24E-03
ODP kg CFC11 eq 5.74E-11 1.12E-15 9.19E-15 2.55E-15 5.59E-16 0 0 -5.21E-11
AP mol H+ eq 2.73E-02 1.28E-05 1.74E-05 1.15E-04 6.4E-06 0 0 -2.46E-02
EP-freshwater kg P eq 5.34E-06 3.14E-08 2.64E-09 7.16E-08 1.57E-08 0 0 -3.21E-06
EP-marine kg N eq 4.3E-03 4.67E-06 5.36E-06 5.6E-05 2.34E-06 0 0 -3.5E-03
EP-terrestrial mol N eq 4.67E-02 5.52E-05 7.6E-05 6.2E-04 2.76E-05 0 0 -3.81E-02
kg NMVOC
POCP 1.31E-02 1.12E-05 1.46E-05 1.49E-04 5.62E-06 0 0 -1.08E-02
eq
ADPE kg Sb eq 2.32E-06 5.66E-10 8.54E-11 1.29E-09 2.83E-10 0 0 -1.75E-06
ADPF MJ 1.04E+02 1.17E-01 2.34E-02 2.67E-01 5.85E-02 0 0 -9.08E+01
m3 world eq
WDP 3.75E-01 1.04E-04 1.07E-02 2.37E-04 5.19E-05 0 0 -2.76E-01
deprived
GWP = Global warming potential; ODP = Depletion potential of the stratospheric ozone layer; AP = Acidification potential of land and water; EP =
Eutrophication potential; POCP = Formation potential of tropospheric ozone photochemical oxidants; ADPE = Abiotic depletion potential for non-fossil
resources; ADPF = Abiotic depletion potential for fossil resources; WDP = Water (user) deprivation potential)
RESULTS OF THE LCA - INDICATORS TO DESCRIBE RESOURCE USE according to EN 15804+A2: 1 kg Schüco Aluminium
Profile
Parameter Unit A1-A3 A4 A5 C1 C2 C3 C4 D
PERE MJ 4.84E+01 8.52E-03 7.88E-01 1.94E-02 4.26E-03 0 0 -4.39E+01
PERM MJ 7.82E-01 0 -7.82E-01 0 0 0 0 0
PERT MJ 4.92E+01 8.52E-03 5.79E-03 1.94E-02 4.26E-03 0 0 -4.39E+01
PENRE MJ 1.04E+02 1.17E-01 3.27E-01 2.68E-01 5.87E-02 0 0 -9.09E+01
PENRM MJ 3.04E-01 0 -3.04E-01 0 0 0 0 0
PENRT MJ 1.04E+02 1.17E-01 2.34E-02 2.68E-01 5.87E-02 0 0 -9.09E+01
SM kg 1.85E-01 0 0 0 0 0 0 1E+00
RSF MJ 0 0 0 0 0 0 0 0
NRSF MJ 0 0 0 0 0 0 0 0
FW m3 8.1E-02 9.33E-06 2.52E-04 2.13E-05 4.66E-06 0 0 -7.63E-02
PERE = Use of renewable primary energy excluding renewable primary energy resources used as raw materials; PERM = Use of renewable primary
energy resources used as raw materials; PERT = Total use of renewable primary energy resources; PENRE = Use of non-renewable primary energy
excluding non-renewable primary energy resources used as raw materials; PENRM = Use of non-renewable primary energy resources used as raw
materials; PENRT = Total use of non-renewable primary energy resources; SM = Use of secondary material; RSF = Use of renewable secondary fuels;
NRSF = Use of non-renewable secondary fuels; FW = Use of net fresh water
RESULTS OF THE LCA – WASTE CATEGORIES AND OUTPUT FLOWS according to EN 15804+A2:
1 kg Schüco Aluminium Profile
Parameter Unit A1-A3 A4 A5 C1 C2 C3 C4 D
HWD kg 6.29E-08 3.64E-13 5.97E-13 8.29E-13 1.82E-13 0 0 -5.76E-08
NHWD kg 1.98E+00 1.79E-05 1.89E-03 4.08E-05 8.95E-06 0 0 -1.88E+00
RWD kg 1.1E-02 2.2E-07 1.31E-06 5.01E-07 1.1E-07 0 0 -1.04E-02
CRU kg 0 0 0 0 0 0 0 0
MFR kg 0 0 1E-04 0 0 1E+00 0 0
MER kg 0 0 0 0 0 0 0 0
EEE MJ 0 0 1.18E-01 0 0 0 0 0
EET MJ 0 0 2.11E-01 0 0 0 0 0
5 Environmental Product Declaration - Schüco International KG - Schüco Aluminium Profile
HWD = Hazardous waste disposed; NHWD = Non-hazardous waste disposed; RWD = Radioactive waste disposed; CRU = Components for re-use;
MFR = Materials for recycling; MER = Materials for energy recovery; EEE = Exported electrical energy; EET = Exported thermal energy
RESULTS OF THE LCA – additional impact categories according to EN 15804+A2-optional:
1 kg Schüco Aluminium Profile
Parameter Unit A1-A3 A4 A5 C1 C2 C3 C4 D
Disease
PM 4.37E-07 1.06E-10 1.07E-10 2.29E-09 5.3E-11 0 0 -3.95E-07
incidence
IR kBq U235 eq 2.21E+00 3.28E-05 2.09E-04 7.47E-05 1.64E-05 0 0 -2.1E+00
ETP-fw CTUe 3.8E+01 8.31E-02 1.1E-02 1.89E-01 4.16E-02 0 0 -3.45E+01
HTP-c CTUh 2.18E-09 1.7E-12 8.97E-13 3.87E-12 8.51E-13 0 0 -1.69E-09
HTP-nc CTUh 8.38E-08 9.07E-11 4.96E-11 2.55E-10 4.54E-11 0 0 -4.5E-08
SQP SQP 1.44E+01 4.89E-02 7.04E-03 1.11E-01 2.45E-02 0 0 -2.67E+00
PM = Potential incidence of disease due to PM emissions; IR = Potential Human exposure efficiency relative to U235; ETP-fw = Potential comparative
Toxic Unit for ecosystems; HTP-c = Potential comparative Toxic Unit for humans (cancerogenic); HTP-nc = Potential comparative Toxic Unit for humans
(not cancerogenic); SQP = Potential soil quality index
Disclaimer 1 – for the indicator “Potential Human exposure efficiency relative to U235”. This impact category deals mainly with the
eventual impact of low-dose ionizing radiation on human health of the nuclear fuel cycle. It does not consider effects due to possible
nuclear accidents, occupational exposure or radioactive waste disposal in underground facilities. Potential ionizing radiation from the
soil, radon and from some construction materials is also not measured by this indicator.
Disclaimer 2 – for the indicators “abiotic depletion potential for non-fossil resources”, “abiotic depletion potential for fossil resources”,
“water (user) deprivation potential, deprivation-weighted water consumption”, “potential comparative toxic unit for ecosystems”,
“potential comparative toxic unit for humans – cancerogenic”, “Potential comparative toxic unit for humans - not cancerogenic”,
“potential soil quality index”. The results of this environmental impact indicator shall be used with care as the uncertainties on these
results are high as there is limited experience with the indicator.
References
Standards list of waste pursuant to Directive 2008/98/EC of the European
Parliament and of the Council.
DIN 4102-4
DIN 4102-4:2016-05, Fire behaviour of building materials and ISO 14025
building components - Part 4: Synopsis and application of EN ISO 14025:2011, Environmental labels and declarations —
classified building materials, components and special Type III environmental declarations — Principles and
components. procedures.
EN 573-3 Regulation (EU) No. 305/2011 (CPR)
EN 573-3:2019-10, Aluminium and aluminium alloys - Chemical REGULATION (EU) No 305/2011 OF THE EUROPEAN
composition and form of wrought products - Part 3: Chemical PARLIAMENT AND OF THE COUNCIL, of 9 March 2011, laying
composition and form of products. down harmonised conditions for the marketing of construction
products and repealing Council Directive 89/106/EEC.
EN 755-1
EN 755-1:2016-10, Aluminium and aluminium alloys – Extruded Schüco Standard 62
rod/bar, tube and profiles –Part 1: Technical conditions for Schüco Standard 62, Technical Delivery Conditions for
inspection and delivery. Extruded Aluminium Profiles.
EN 1090-3 Further References
EN1090-3:2019, Execution of steel structures and aluminium
structures - Part 3: Technical requirements for aluminium EPD: Aluminiumprofil pressblank
structures. Umwelt-Produktdeklaration: Aluminiumprofil pressblank.
Aluminium Deutschland, EPD-GDA-20190068-IBH2-DE. Berlin:
EN 12020-1 Institut Bauen und Umwelt e.V. (Hrsg.), 13.11.2019.
EN 12020-1:2022, Aluminium and aluminium alloys - Extruded
precision profiles in alloys EN AW-6060 and EN AW-6063 - Part IBU 2021
1: Technical conditions for inspection and delivery. Institut Bauen und Umwelt e.V.: General Instructions for the
EPD programme of Institut Bauen und Umwelt e.V., Version
EN 15088 2.0, Berlin: Institut Bauen und Umwelt e.V., https://ibu-
EN 15088:2006-03, Aluminium and aluminium alloys – epd.com/, 2021.
Structural products for construction works –Technical conditions
for inspection and delivery. IBU PCR Part A
PCR - Part A: Calculation Rules for the Life Cycle Assessment
EN 15804 and Requirements on the Project Report according to EN
EN15804:2012+A2:2019+AC:2021, Sustainability of 15804+A2:2019, version 1.3, Institut Bauen und Umwelt e.V.,
construction works — Environmental Product Declarations — https://ibu-epd.com/, 2022.
Core rules for the product category of construction products.
IBU PCR Part B
EWC PCR – Part B: Requirements of the EPD for products of
European Waste Catalogue (EWC), COMMISSION DECISION aluminium and aluminium alloys, version 7, 24/07/2023, Institut
of 18 December 2014 amending Decision 2000/532/EC on the Bauen und Umwelt e.V., https://ibu-epd.com/, 2021.
6 Environmental Product Declaration - Schüco International KG - Schüco Aluminium Profile
https://sphera.com/product-sustainability-gabi-data-search/,
LCAfE software and MLC databases 2023.
LCAfE and MLC databases (f.k.a. GaBi) by Sphera. Version
CUP 2023.1. Sphera Solutions GmbH,
7 Environmental Product Declaration - Schüco International KG - Schüco Aluminium Profile
Publisher
Institut Bauen und Umwelt e.V. +49 (0)30 3087748- 0
Hegelplatz 1 info@ibu-epd.com
10117 Berlin www.ibu-epd.com
Germany
Programme holder
Institut Bauen und Umwelt e.V. +49 (0)30 3087748- 0
Hegelplatz 1 info@ibu-epd.com
10117 Berlin www.ibu-epd.com
Germany
Author of the Life Cycle Assessment
Sphera Solutions GmbH +49 (0)711 341817-0
Hauptstraße 111- 113 info@sphera.com
70771 Leinfelden-Echterdingen www.sphera.com
Germany
Owner of the Declaration
Schüco International KG +49 (0)521 78 30
Karolinenstraße 1-15 info@schueco.com
33609 Bielefeld www.schueco.com
Germany
8 Environmental Product Declaration - Schüco International KG - Schüco Aluminium Profile
