ENVIRONMENTAL PRODUCT DECLARATION
as per ISO 14025 and EN 15804+A2
Owner of the Declaration Sika Limited
Publisher Institut Bauen und Umwelt e.V. (IBU)
Programme holder Institut Bauen und Umwelt e.V. (IBU)
Declaration number EPD-SIK-20240171-CBA2-EN
Issue date 20/06/2024
Valid to 19/06/2029
SikaRapid®-800 ECO
Sika Limited
www.ibu-epd.com | https://epd-online.com
General Information
Sika Limited SikaRapid®-800 ECO
Programme holder Owner of the declaration
IBU – Institut Bauen und Umwelt e.V. Sika Limited
Hegelplatz 1 Watchmead Site C
10117 Berlin AL7 1BQ Welwyn Garden City
Germany United Kingdom
Declaration number Declared product / declared unit
EPD-SIK-20240171-CBA2-EN The EPD refers to the declared unit of 1 kg of concrete admixture
(hardening accelerator) with a density of 1.19 g/ml applied into the building
in accordance with IBU PCR 04-2023 part B.
This declaration is based on the product category rules: Scope:
Concrete admixtures, 01/08/2021 This core-EPD relates to 1 kg of SikaRapid®-800 ECO, (a hardening
(PCR checked and approved by the SVR) accelerating admixture according to BS EN 934-2:2009+A1:2012),
manufactured at Sika's plant in Watchmead, Welwyn Garden City, AL7
1BQ, United Kingdom and is representative for the year 2022.
Issue date The results in this core-EPD were calculated using an LCA-tool verified by
IBU in 2023.
20/06/2024
The owner of the declaration shall be liable for the underlying information
and evidence; the IBU shall not be liable with respect to manufacturer
information, life cycle assessment data and evidences.
Valid to
19/06/2029 The EPD was created according to the specifications of EN 15804+A2. In
the following, the standard will be simplified as EN 15804.
Verification
The standard EN 15804 serves as the core PCR
Independent verification of the declaration and data according to ISO
14025:2011
internally X externally
Dipl.-Ing. Hans Peters
(Chairman of Institut Bauen und Umwelt e.V.)
Florian Pronold Matthias Schulz,
(Managing Director Institut Bauen und Umwelt e.V.) (Independent verifier)
1 Environmental Product Declaration - Sika Limited - SikaRapid®-800 ECO
Product
Additional technical data are not relevant for this product.
Product description/Product definition
SikaRapid®-800 ECO is a liquid hardening accelerator for Performance data of the product in accordance with the
concrete and mortar, designed specifically for enhancing the declaration of performance with respect to its essential
performance of concrete with high levels of supplementary characteristics according to BS EN 934-2:2009+A1:2012,
cementitious material (SCM), such as GGBS and PFA. It Admixtures for concrete, mortar and grout – Part 2: Concrete
promotes early and late age strength development without admixtures – Definitions, requirements, conformity, marking and
negatively influencing final strengths. labelling.
For the purposes of this EPD, Sika's Watchmead, Welwyn
Garden City, AL7 1BQ manufacturing site was selected. The Base materials/Ancillary materials
product needs a declaration of performance taking into The raw materials and additives of SikaRapid®-800 ECO can
consideration BS EN 934-2:2009+A1:2012, Admixtures for be given as follows:
concrete, mortar and grout – Part 2: Concrete admixtures – Name Value Unit
Definitions, requirements, conformity, marking and labelling and
Water 40-60 %
the CE- marking. For the application and use the respective
Sodium Nitrate 10-20 %
national provisions apply.
Sodium Thiocyanate 10-20 %
Application Lactic Acid 3-5 %
SikaRapid®-800 ECO is used as a constituent material to
2,2'-iminodiethanol 0.1-0.5 %
produce concrete. It can be used in combination with other Sika
2-octyl-2H-isothiazole-3-one (OIT) 0.0002-0.0015 %
admixtures and can be successfully used in mix designs
Additives 5-15 %
utilizing supplementary cementitious materials.
This product contains substances listed in the candidate list
Technical Data
(date: 20.04.2023) exceeding 0.1 percentage by mass: No
SikaRapid®-800 ECO meets the requirements of BS EN 934-
This product contains other CMR substances in categories 1A
2:2009+A1:2012, Table 7.
or 1B which are not on the candidate list, exceeding 0.1
Constructional data percentage by mass: No
Biocide products were added to this construction product or it
Name Value Unit
has been treated with biocide products (this then concerns a
Chloride content
0.1 M.-% treated product as defined by the (EU) Ordinance on Biocide
(EN 480-10)
Products Number 528/2012): Yes
Alkali content (EN
10 M.-%
480-12)
Please refer to most recent Safety Datasheet for further details.
Corrosion
Contains the following components
behavior (EN μ Reference service life
from EN 934-1 Annex A.2:
934-1 / EN 480- A/cm2 The durability of concreate admixtures is normally at least as
Thiocyanates, nitrates
14) long as the lifetime of the building in which it is used. The
Air content of documentation of the RSL is not required for the EPDs
fresh concrete Test mix ≤ 2 % by volume above Vol.-% calculated using the EPD tool from Sika since the entire life
(EN 12350-7) control mix cycle is not declared. Only modules A1-A3, A4, A5, C1, C2, C4
and D are considered.
At 20° C and 24 h: test mix ≥ 120 %
Compressive of control mix; at 20° C and 28 days:
strength (EN test mix ≥ 90 % of control mix; at 5° N/mm2
12390-3) C and 48 h: test mix ≥ 130 % of
control mix
LCA: Calculation rules
Declared Unit System boundary
The EPD refers to the declared unit of 1kg of concrete Declaration type with respect to life cycle stages covered
admixture (hardening accelerator) applied into the building with according to clause 5.2 EN 15804+A2 is cradle to gate with
a density of 1.19 g/ml in accordance with IBU PCR 04-2023 modules C1–C4 and module D (A1–A3, A4, A5, C and D).
part B. Modules taken into account:
Declared unit and mass reference • A1 Production of preliminary products
Name Value Unit • A2 Transport to the plant
• A3 Production including provision of energy, production
Declared unit 1 kg
of auxiliaries and consumables and waste treatment
Gross density 1191 kg/m3
• A4 Transport from the construction site to the installation
Other declared units are allowed if the conversion is shown site (weighted average distance calculated on deliveries
transparently. of this product from 2022-23)
• A5 Installation, admixtures applied into the building
LCA values take into account 12 months of detailed production during A5 phase operations. At this stage, an impact of
site data from 2022 and are presented with a high degree of the production and treatment of installation residue
confidence. equal to 1% of the product is considered.
2 Environmental Product Declaration - Sika Limited - SikaRapid®-800 ECO
• C1-C2-C4-D A5.
The building deconstruction (demolition process) takes
place in C1 module which considers energy production Geographic Representativeness
and consumption in terms of diesel and all the Land or region, in which the declared product system is
emissions connected with the fuel-burning process. manufactured, used or handled at the end of the product´s
After the demolition, the admixture is transported to the lifespan: United Kingdom
end-of-life processing (C2 module) where all the
impacts related to the transport processes are
Comparability
considered.
Basically, a comparison or an evaluation of EPD data is only
• One scenario is considered for the final treatment of the
possible if all the data sets to be compared were created
waste:
according to EN 15804 and the building context, respectively
100% disposal (C4), modelled by landfill process where
the product-specific characteristics of performance, are taken
admixtures end their life cycle.
into account. Sphera LCA for Expert software (version 10) and
Module D accounts for benefits that are beyond the
Managed LCA Content (2022.2) have been used.
defined system boundaries. Credits are generated
during the incineration of the wooden pallets in module
LCA: Scenarios and additional technical information
Characteristic product properties of biogenic carbon
No biogenic carbon is contained in the product.
Information on describing the biogenic carbon content at Assembly (A5)
factory gate
Name Value Unit
Name Value Unit
Other resources - kg
kg
Biogenic carbon content in product - Material loss 0.01 kg
C
Biogenic carbon content in accompanying kg End of life (C1-C4)
0.0076
packaging C C1: This module considers the use of machinery (7.5E-5 kg of
diesel for kg handled) to dismantle the product to enable its
Note: 1 kg of biogenic carbon is equivalent to 44/12 kg of CO .
2 subsequent transport.
C2: The concrete demolition waste is transported from the
building site to a treatment plant or disposal site by truck and
an average distance of 50 km is considered.
Transport from the gate to the site (A4) C4: The results for the end-of-life are declared for one scenario:
Name Value Unit Name Value Unit
Transport distance weighted average 176.3 km Landfill percentage 100 %
Material to landfill 1 kg
3 Environmental Product Declaration - Sika Limited - SikaRapid®-800 ECO
LCA: Results
DESCRIPTION OF THE SYSTEM BOUNDARY (X = INCLUDED IN LCA; MND = MODULE OR INDICATOR NOT DECLARED; MNR
= MODULE NOT RELEVANT)
Benefits and
Construction loads beyond
Product stage Use stage End of life stage
process stage the system
boundaries
la ire ta m w a Ry lp p u s tro p s n a rT g n iru tc a fu n a M e h t m o rf tro p s n a rTe tis e h t o t e ta g y lb m e s s A e s U e c n a n e tn ia M ria p e R tn e m e c a lp e R tn e m h s ib ru fe R y g re n e la n o ita re p Oe s u re ta w la n o ita re p Oe s u n o itc u rts n o c -e Dn o itilo m e d tro p s n a rT g n is s e c o rp e ts a W la s o p s iD -e s u e R-y re v o c e R-g n ilc y c e Rla itn e to p
A1 A2 A3 A4 A5 B1 B2 B3 B4 B5 B6 B7 C1 C2 C3 C4 D
X X X X X MND MND MNR MNR MNR MND MND X X MND X X
RESULTS OF THE LCA - ENVIRONMENTAL IMPACT according to EN 15804+A2: 1 kg SikaRapid-800 ECO
Parameter Unit A1-A3 A4 A5 C1 C2 C4 D
GWP-total kg CO 2 eq 1.06E+00 9.11E-03 9.29E-02 2.83E-04 6.27E-03 1.45E-02 -3.28E-02
GWP-fossil kg CO 2 eq 1.14E+00 8.71E-03 5.7E-02 2.7E-04 6E-03 1.49E-02 -3.26E-02
GWP-biogenic kg CO 2 eq -8.62E-02 3.94E-04 3.59E-02 1.23E-05 2.71E-04 -4.42E-04 -1.66E-04
GWP-luluc kg CO 2 eq 2.38E-04 3.96E-07 2.45E-06 1.25E-08 2.72E-07 2.75E-05 -3.56E-06
ODP kg CFC11 eq 2.02E-12 8.95E-16 2.59E-14 2.82E-17 6.15E-16 3.51E-14 -2.19E-13
AP mol H+ eq 2.53E-03 2.54E-05 4.11E-05 3.62E-06 1.91E-05 1.06E-04 -4.27E-05
EP-freshwater kg P eq 1.8E-05 2.04E-09 1.81E-07 6.41E-11 1.4E-09 2.53E-08 -4.45E-08
EP-marine kg N eq 8.21E-04 1.17E-05 1.27E-05 1.65E-06 8.89E-06 2.71E-05 -1.16E-05
EP-terrestrial mol N eq 8.26E-03 1.29E-04 1.51E-04 1.81E-05 9.78E-05 2.97E-04 -1.24E-04
kg NMVOC
POCP 1.63E-03 2.36E-05 2.85E-05 4.95E-06 1.77E-05 8.22E-05 -3.25E-05
eq
ADPE kg Sb eq 3.09E-07 4.57E-10 3.03E-09 1.44E-11 3.14E-10 1.53E-09 -4.89E-09
ADPF MJ 2.13E+01 1.22E-01 2.33E-01 3.84E-03 8.39E-02 1.95E-01 -5.54E-01
m3 world eq
WDP 3.38E-01 2.36E-05 1.2E-02 7.43E-07 1.62E-05 1.64E-03 -3.44E-03
deprived
GWP = Global warming potential; ODP = Depletion potential of the stratospheric ozone layer; AP = Acidification potential of land and water; EP =
Eutrophication potential; POCP = Formation potential of tropospheric ozone photochemical oxidants; ADPE = Abiotic depletion potential for non-fossil
resources; ADPF = Abiotic depletion potential for fossil resources; WDP = Water (user) deprivation potential)
RESULTS OF THE LCA - INDICATORS TO DESCRIBE RESOURCE USE according to EN 15804+A2: 1 kg SikaRapid-800 ECO
Parameter Unit A1-A3 A4 A5 C1 C2 C4 D
PERE MJ 2.97E+00 7.39E-04 2.65E-01 2.33E-05 5.08E-04 2.93E-02 -1.51E-01
PERM MJ 2.29E-01 0 -2.29E-01 0 0 0 0
PERT MJ 3.2E+00 7.39E-04 3.56E-02 2.33E-05 5.08E-04 2.93E-02 -1.51E-01
PENRE MJ 1.93E+01 1.23E-01 7.93E-01 3.86E-03 8.42E-02 1.96E-01 -5.54E-01
PENRM MJ 1.98E+00 0 -5.6E-01 0 0 0 0
PENRT MJ 2.13E+01 1.23E-01 2.33E-01 3.86E-03 8.42E-02 1.96E-01 -5.54E-01
SM kg 0 0 0 0 0 0 0
RSF MJ 0 0 0 0 0 0 0
NRSF MJ 0 0 0 0 0 0 0
FW m3 1.64E-02 1E-06 3.67E-04 3.16E-08 6.9E-07 4.97E-05 -1.45E-04
PERE = Use of renewable primary energy excluding renewable primary energy resources used as raw materials; PERM = Use of renewable primary
energy resources used as raw materials; PERT = Total use of renewable primary energy resources; PENRE = Use of non-renewable primary energy
excluding non-renewable primary energy resources used as raw materials; PENRM = Use of non-renewable primary energy resources used as raw
materials; PENRT = Total use of non-renewable primary energy resources; SM = Use of secondary material; RSF = Use of renewable secondary fuels;
NRSF = Use of non-renewable secondary fuels; FW = Use of net fresh water
RESULTS OF THE LCA – WASTE CATEGORIES AND OUTPUT FLOWS according to EN 15804+A2:
1 kg SikaRapid-800 ECO
Parameter Unit A1-A3 A4 A5 C1 C2 C4 D
HWD kg 2.9E-05 4.23E-13 2.9E-07 1.33E-14 2.91E-13 1.01E-11 -7.53E-11
NHWD kg 3.71E-02 1.25E-05 1.91E-03 3.94E-07 8.6E-06 1E+00 -2.79E-04
RWD kg 3.69E-04 2.02E-07 4.57E-06 6.36E-09 1.39E-07 2.18E-06 -4.33E-05
CRU kg 0 0 0 0 0 0 0
MFR kg 0 0 0 0 0 0 0
MER kg 0 0 0 0 0 0 0
EEE MJ 0 0 1.45E-01 0 0 0 0
EET MJ 0 0 2.66E-01 0 0 0 0
HWD = Hazardous waste disposed; NHWD = Non-hazardous waste disposed; RWD = Radioactive waste disposed; CRU = Components for re-use;
MFR = Materials for recycling; MER = Materials for energy recovery; EEE = Exported electrical energy; EET = Exported thermal energy
4 Environmental Product Declaration - Sika Limited - SikaRapid®-800 ECO
RESULTS OF THE LCA – additional impact categories according to EN 15804+A2-optional:
1 kg SikaRapid-800 ECO
Parameter Unit A1-A3 A4 A5 C1 C2 C4 D
Disease
PM ND ND ND ND ND ND ND
incidence
IR kBq U235 eq ND ND ND ND ND ND ND
ETP-fw CTUe ND ND ND ND ND ND ND
HTP-c CTUh ND ND ND ND ND ND ND
HTP-nc CTUh ND ND ND ND ND ND ND
SQP SQP ND ND ND ND ND ND ND
PM = Potential incidence of disease due to PM emissions; IR = Potential Human exposure efficiency relative to U235; ETP-fw = Potential comparative
Toxic Unit for ecosystems; HTP-c = Potential comparative Toxic Unit for humans (cancerogenic); HTP-nc = Potential comparative Toxic Unit for humans
(not cancerogenic); SQP = Potential soil quality index
The additional and optional impact categories according to EN 15804+A2 are not declared, as the uncertainty of these indicators is to
be classified as high.
Disclaimer 1 – for the indicator 'Potential Human exposure efficiency relative to U235'. This impact category deals mainly with the
eventual impact of low-dose ionizing radiation on human health of the nuclear fuel cycle. It does not consider effects due to possible
nuclear accidents, occupational exposure or radioactive waste disposal in underground facilities. Potential ionizing radiation from the
soil, radon and from some construction materials is also not measured by this indicator.
Disclaimer 2 – for the indicators 'abiotic depletion potential for non-fossil resources', 'abiotic depletion potential for fossil resources',
'water (user) deprivation potential, deprivation-weighted water consumption', 'potential comparative toxic unit for ecosystems', 'potential
comparative toxic unit for humans – cancerogenic', 'Potential comparative toxic unit for humans - not cancerogenic', 'potential soil
quality index'. The results of this environmental impact indicator shall be used with care as the uncertainties on these results are high
as there is limited experience with the indicator.
This EPD was created using a software tool.
References
EN 934-2 2.0, Berlin: Institut Bauen und Umwelt e.V., 2021 www.ibu-
BS EN 934-2+A1:2012. Admixtures for concrete, mortar and epd.com
grout, Part2: Concrete admixtures - Definitions, requirements,
conformity, marking and labelling LCA Calculator
LCA Calculator software (version 6). Visualize, Improve and
EN 480-10 Report on Product Sustainability. https://sphera.com/your-path-
Admixtures for concrete, mortar and grout. Test methods. to-sustainability/
Determination of water soluble chloride content
LCA for Experts
EN 15804 Life cycle assessment software (version 10), by Sphera
EN 15804:2012+A1:2013, Sustainability of construction works Solutions GmbH, Leinfelden-Echterdingen, 2022
— Environmental Product Declarations — Core rules for the https://sphera.com/life-cycle-assessment-lca-software/
product category of construction products.
Managed LCA Content
EN 15804 Life cycle assessment database, by Sphera Solutions GmbH,
EN 15804:2012+A2:2019+AC:2021, Sustainability of Leinfelden-Echterdingen, 2022, https://sphera.com/life-cycle-
construction works — Environmental Product Declarations — assessment-lca-database/
Core rules for the product category of construction products.
PCR Part A
ISO 14025 PCR - Part A: Calculation rules for the Life Cycle Assessment
EN ISO 14025:2011, Environmental labels and declarations — and Requirements on the Background Report, version 1.3,
Type III environmental declarations — Principles and Institut Bauen und Umwelt e.V., 08-2021.
procedures.
IBU 2021 PCR Part B
Institut Bauen und Umwelt e.V.: General Instructions for the PCR – Part B:Requirements on the EPD for Concrete
EPD programme of Institut Bauen und Umwelt e.V., Version admixtures, Institut Bauen und Umwelt e.V., 04-2023.
5 Environmental Product Declaration - Sika Limited - SikaRapid®-800 ECO
Publisher
Institut Bauen und Umwelt e.V. +49 (0)30 3087748- 0
Hegelplatz 1 info@ibu-epd.com
10117 Berlin www.ibu-epd.com
Germany
Programme holder
Institut Bauen und Umwelt e.V. +49 (0)30 3087748- 0
Hegelplatz 1 info@ibu-epd.com
10117 Berlin www.ibu-epd.com
Germany
Author of the Life Cycle Assessment
Sika Limited +44 1707 394444
Watchmead Site C concrete@uk.sika.com
AL7 1BQ Welwyn Garden City https://gbr.sika.com/
United Kingdom
Owner of the Declaration
Sika Limited +44 1707 394444
Watchmead Site C concrete@uk.sika.com
AL7 1BQ Welwyn Garden City https://gbr.sika.com/
United Kingdom
6 Environmental Product Declaration - Sika Limited - SikaRapid®-800 ECO
