ENVIRONMENTAL PRODUCT DECLARATION
as per ISO 14025 and EN 15804+A2
Owner of the Declaration SIKA HELLAS ABEE
Publisher Institut Bauen und Umwelt e.V. (IBU)
Programme holder Institut Bauen und Umwelt e.V. (IBU)
Declaration number EPD-SIK-20240179-CBA2-EN
Issue date 20/06/2024
Valid to 19/06/2029
SikaTard®-930
Sika Hellas ABEE
www.ibu-epd.com | https://epd-online.com
General Information
Sika Hellas ABEE SikaTard®-930
Programme holder Owner of the declaration
IBU – Institut Bauen und Umwelt e.V. SIKA HELLAS ABEE
Hegelplatz 1 PROTOMAGIAS STR. 15
10117 Berlin 14568 athens
Germany Greece
Declaration number Declared product / declared unit
EPD-SIK-20240179-CBA2-EN 1 kg of SikaTard®-930 with a density of 1.12 g/ml.
This declaration is based on the product category rules: Scope:
Concrete admixtures, 01/08/2021 This core-EPD relates to 1kg of SikaTard®-930 (admixture group Retarder)
(PCR checked and approved by the SVR) applied into the building, manufactured at Sika's plant in Sika Hellas
Kalochori 57009,Thessaloniki and is representative for the year 2022.
The results in this core-EPD were calculated using an LCA-tool verified by
Issue date IBU in 2023.
20/06/2024
The owner of the declaration shall be liable for the underlying information
and evidence; the IBU shall not be liable with respect to manufacturer
information, life cycle assessment data and evidences.
Valid to
19/06/2029 The EPD was created according to the specifications of EN 15804+A2. In
the following, the standard will be simplified as EN 15804.
Verification
The standard EN 15804 serves as the core PCR
Independent verification of the declaration and data according to ISO
14025:2011
internally X externally
Dipl.-Ing. Hans Peters
(Chairman of Institut Bauen und Umwelt e.V.)
Florian Pronold Matthias Schulz,
(Managing Director Institut Bauen und Umwelt e.V.) (Independent verifier)
1 Environmental Product Declaration - Sika Hellas ABEE - SikaTard®-930
Product
Additional technical data are not relevant for this product.
Product description/Product definition
SikaTard®-930 is an admixture developed for the control of Performance data of the product in accordance with the
cement hydration. SikaTard®-930 stabilises concrete mixes declaration of performance with respect to its essential
without setting for extended periods and without negatively characteristics according to EN 934-2:2009+Α1:2012,
influencing their quality. Admixtures for concrete, mortar and grout – Part 2: Concrete
admixtures – Definitions, requirements, conformity, marking and
labelling.
The product needs a declaration of performance taking into
consideration EN 934-2:2009+Α1:2012, Admixtures for Base materials/Ancillary materials
concrete, mortar and grout – Part 2: Concrete admixtures – The raw materials and additives of SikaTard®-930 can be given
Definitions, requirements, conformity, marking and labelling and as follows:
the CE- marking. For the application and use the respective • Water: 60 – 70%
national provisions apply. • Phosphate: 20 – 30%
• Additives: 0.5 - 10%
Application
SikaTard®-930 finds its primary application in both wet and dry This product contains substances listed in the candidate list
spray shotcrete, serving to delay the cement hydration process (date: 20.04.2023) exceeding 0.1 percentage by mass: No
until needed. This capability allows for the stabilization of mixed This product contains other CMR substances in categories 1A
concrete over extended periods, spanning hours or even days, or 1B which are not on the candidate list, exceeding 0.1
ideal for applications such as tunnelling projects. SikaTard®- percentage by mass: No
930 is mainly used in wet and dry spray shotcrete where Biocide products were added to this construction product or it
cement hydration of the concrete mix is prevented until it is has been treated with biocide products (this then concerns a
required. It is therefore possible to stabilise mixed concrete for treated product as defined by the (EU) Ordinance on Biocide
hours or even days i.e. in tunnelling work. The product needs a Products No. 528/2012): Yes (In can preservative: 2-Octyl-2H-
declaration of performance taking into consideration EN 934- isothiazol-3-one (26530-20-1), (Ethylenedioxy)dimethanol
2:2009+Α1:2012, Admixtures for concrete, mortar and grout – (3586-55-8).
Part 2: Concrete admixtures – Definitions, requirements,
conformity, marking and labelling and the CE- marking. For the
application and use the respective national provisions apply.
Technical Data
SikaTard®-930 is set according to EN 934-2:2009+Α1:2012, Reference service life
Admixtures for concrete, mortar and grout – Part 2: Concrete The durability of concrete admixtures is normally at least as
admixtures – Definitions, requirements, conformity, marking and long as the lifetime of the building in which it is used. The
labelling, Declaration of Performance 20929148 and provided experimental data show that the reference life is greater than
with the CE Marking. 50 years.
Constructional data The documentation of the RSL is not required for the EPDs
calculated using the EPD tool from Sika since the entire life
Name Value Unit
cycle is not declared. Only modules A1-A3, A4, A5, C1-C4 and
Density (ISO 758) 1.12 g/ml
D are considered
pH value (ISO 4316) 3 -log 10(a H+)
LCA: Calculation rules
• A5 Installation, admixtures applied into the building during A5
Declared Unit phase operations. At this stage, an impact of the production
The EPD refers to the declared unit of 1kg of concrete and treatment of installation residue equal to 1% of the product
admixture (retarder) applied into the building with a density of is considered.
1.12 g/ml in accordance with IBU PCR 04-2023 part B • C1-C2-C4-D
Declared unit and mass reference The building deconstruction (demolition process) takes place in
C1 module which considers energy production and
Name Value Unit
consumption in terms of diesel and all the emissions connected
Declared unit 1 kg
with the fuel-burning process. After the demolition, the
Gross density 1120 kg/m3 admixture is transported to the end-of-life processing (C2
module) where all the impacts related to the transport
System boundary processes are considered.
Declaration type with respect to life cycle stages covered One scenario is considered for the final treatment of the waste:
according to clause 5.2 EN 15804+A2 is cradle to gate with • 100% disposal (C4), modelled by landfill process where
modules C1–C4 and module D (A1–A3, A4, A5, C and D). admixtures end their life cycle.
Modules taken into account: Module D accounts for benefits that are beyond the defined
• A1 Production of preliminary products system boundaries. Credits are generated during the
• A2 Transport to the plant incineration of the installation scrap in module A5.
• A3 Production including provision of energy, production of
Geographic Representativeness
auxiliaries and consumables and waste treatment
Land or region, in which the declared product system is
• A4 Transport from the construction site to the installation site
manufactured, used or handled at the end of the product´s
2 Environmental Product Declaration - Sika Hellas ABEE - SikaTard®-930
lifespan: Greece according to EN 15804 and the building context, respectively
the product-specific characteristics of performance, are taken
into account. Sphera LCA for Expert software (version 10) and
Comparability
Managed LCA Content (2022.2) have been used.
Basically, a comparison or an evaluation of EPD data is only
possible if all the data sets to be compared were created
LCA: Scenarios and additional technical information
Material loss regards the amount of product not used during the
Characteristic product properties of biogenic carbon application phase into the building. This amount is 1 % of the
No biogenic carbon is contained in the product. product, impacts related to the production of this part are
Information on describing the biogenic carbon content at charged to the A5 module. This percentage is considered as
factory gate waste to incineration since the product has a calorific value and
impacts of its end of life have been considered in the LCA
Name ValueUnit
model and declared in A5.
kg
Biogenic carbon content in product -
C
End of life (C1-C4)
Biogenic carbon content in accompanying kg
- C1: This module considers the use of machinery (7.5E-5 kg of
packaging C
diesel for kg handled) to dismantle the product to enable its
Note: 1 kg of biogenic carbon is equivalent to 44/12 kg of CO 2. subsequent transport.
C2: The concrete demolition waste is transported from the
building site to a treatment plant or disposal site by truck and
an average distance of 50 km is considered.
C4: The results for the end-of-life are declared for one scenario:
Transport from the gate to the side (A4)
Name Value Unit
Name Value Unit
Landfill percentage 100 %
Transport distance 300 km
Landfilling 1 kg
Assembly (A5)
Name Value Unit
Material loss 0.01 kg
Other resources - kg
3 Environmental Product Declaration - Sika Hellas ABEE - SikaTard®-930
LCA: Results
DESCRIPTION OF THE SYSTEM BOUNDARY (X = INCLUDED IN LCA; MND = MODULE OR INDICATOR NOT DECLARED; MNR
= MODULE NOT RELEVANT)
Benefits and
Construction loads beyond
Product stage Use stage End of life stage
process stage the system
boundaries
la ire ta m w a Ry lp p u s tro p s n a rT g n iru tc a fu n a M e h t m o rf tro p s n a rTe tis e h t o t e ta g y lb m e s s A e s U e c n a n e tn ia M ria p e R tn e m e c a lp e R tn e m h s ib ru fe R y g re n e la n o ita re p Oe s u re ta w la n o ita re p Oe s u n o itc u rts n o c -e Dn o itilo m e d tro p s n a rT g n is s e c o rp e ts a W la s o p s iD -e s u e R-y re v o c e R-g n ilc y c e Rla itn e to p
A1 A2 A3 A4 A5 B1 B2 B3 B4 B5 B6 B7 C1 C2 C3 C4 D
X X X X X MND MND MNR MNR MNR MND MND X X MND X X
RESULTS OF THE LCA - ENVIRONMENTAL IMPACT according to EN 15804+A2: 1 kg SikaTard®-930
Parameter Unit A1-A3 A4 A5 C1 C2 C4 D
GWP-total kg CO 2 eq 1.9E+00 1.51E-02 2.24E-02 2.83E-04 6.27E-03 1.45E-02 -1.48E-03
GWP-fossil kg CO 2 eq 1.88E+00 1.44E-02 2.22E-02 2.7E-04 6E-03 1.49E-02 -1.48E-03
GWP-biogenic kg CO 2 eq 1.7E-02 6.51E-04 1.65E-04 1.23E-05 2.71E-04 -4.42E-04 -7.58E-06
GWP-luluc kg CO 2 eq 7.54E-04 6.55E-07 7.82E-06 1.25E-08 2.72E-07 2.75E-05 -1.63E-07
ODP kg CFC11 eq 1.46E-11 1.48E-15 1.47E-13 2.82E-17 6.15E-16 3.51E-14 -1E-14
AP mol H+ eq 3.45E-03 4.2E-05 3.63E-05 3.62E-06 1.91E-05 1.06E-04 -1.95E-06
EP-freshwater kg P eq 2.35E-05 3.37E-09 2.36E-07 6.41E-11 1.4E-09 2.53E-08 -2.04E-09
EP-marine kg N eq 1.1E-03 1.93E-05 1.15E-05 1.65E-06 8.89E-06 2.71E-05 -5.28E-07
EP-terrestrial mol N eq 1.16E-02 2.12E-04 1.23E-04 1.81E-05 9.78E-05 2.97E-04 -5.65E-06
kg NMVOC
POCP 2.93E-03 3.9E-05 3.07E-05 4.95E-06 1.77E-05 8.22E-05 -1.48E-06
eq
ADPE kg Sb eq 8.23E-07 7.56E-10 8.25E-09 1.44E-11 3.14E-10 1.53E-09 -2.24E-10
ADPF MJ 3.16E+01 2.02E-01 3.2E-01 3.84E-03 8.39E-02 1.95E-01 -2.51E-02
m3 world eq
WDP 3.62E-01 3.9E-05 3.92E-03 7.43E-07 1.62E-05 1.64E-03 -1.58E-04
deprived
GWP = Global warming potential; ODP = Depletion potential of the stratospheric ozone layer; AP = Acidification potential of land and water; EP =
Eutrophication potential; POCP = Formation potential of tropospheric ozone photochemical oxidants; ADPE = Abiotic depletion potential for non-fossil
resources; ADPF = Abiotic depletion potential for fossil resources; WDP = Water (user) deprivation potential)
RESULTS OF THE LCA - INDICATORS TO DESCRIBE RESOURCE USE according to EN 15804+A2: 1 kg SikaTard®-930
Parameter Unit A1-A3 A4 A5 C1 C2 C4 D
PERE MJ 9.32E+00 1.22E-03 9.36E-02 2.33E-05 5.08E-04 2.93E-02 -6.94E-03
PERM MJ 0 0 0 0 0 0 0
PERT MJ 9.32E+00 1.22E-03 9.36E-02 2.33E-05 5.08E-04 2.93E-02 -6.94E-03
PENRE MJ 3.16E+01 2.03E-01 3.64E-01 3.86E-03 8.42E-02 1.96E-01 -2.51E-02
PENRM MJ 4.3E-02 0 -4.3E-02 0 0 0 0
PENRT MJ 3.16E+01 2.03E-01 3.21E-01 3.86E-03 8.42E-02 1.96E-01 -2.51E-02
SM kg 0 0 0 0 0 0 0
RSF MJ 0 0 0 0 0 0 0
NRSF MJ 0 0 0 0 0 0 0
FW m3 2.03E-02 1.66E-06 2.1E-04 3.16E-08 6.9E-07 4.97E-05 -6.67E-06
PERE = Use of renewable primary energy excluding renewable primary energy resources used as raw materials; PERM = Use of renewable primary
energy resources used as raw materials; PERT = Total use of renewable primary energy resources; PENRE = Use of non-renewable primary energy
excluding non-renewable primary energy resources used as raw materials; PENRM = Use of non-renewable primary energy resources used as raw
materials; PENRT = Total use of non-renewable primary energy resources; SM = Use of secondary material; RSF = Use of renewable secondary fuels;
NRSF = Use of non-renewable secondary fuels; FW = Use of net fresh water
RESULTS OF THE LCA – WASTE CATEGORIES AND OUTPUT FLOWS according to EN 15804+A2:
1 kg SikaTard®-930
Parameter Unit A1-A3 A4 A5 C1 C2 C4 D
HWD kg 3.02E-09 6.99E-13 3.04E-11 1.33E-14 2.91E-13 1.01E-11 -3.4E-12
NHWD kg 3.56E-02 2.07E-05 1.04E-02 3.94E-07 8.6E-06 1E+00 -1.27E-05
RWD kg 1.19E-03 3.34E-07 1.2E-05 6.36E-09 1.39E-07 2.18E-06 -1.99E-06
CRU kg 0 0 0 0 0 0 0
MFR kg 0 0 0 0 0 0 0
MER kg 0 0 0 0 0 0 0
EEE MJ 0 0 6.68E-03 0 0 0 0
EET MJ 0 0 1.19E-02 0 0 0 0
HWD = Hazardous waste disposed; NHWD = Non-hazardous waste disposed; RWD = Radioactive waste disposed; CRU = Components for re-use;
MFR = Materials for recycling; MER = Materials for energy recovery; EEE = Exported electrical energy; EET = Exported thermal energy
4 Environmental Product Declaration - Sika Hellas ABEE - SikaTard®-930
RESULTS OF THE LCA – additional impact categories according to EN 15804+A2-optional:
1 kg SikaTard®-930
Parameter Unit A1-A3 A4 A5 C1 C2 C4 D
Disease
PM 3.31E-08 2.41E-10 3.48E-10 1.93E-10 1.06E-10 1.3E-09 -1.61E-11
incidence
IR kBq U235 eq 1.58E-01 5.01E-05 1.59E-03 9.55E-07 2.08E-05 2.42E-04 -3.37E-04
ETP-fw CTUe 1.39E+01 1.44E-01 1.43E-01 2.74E-03 5.97E-02 1.1E-01 -5.55E-03
HTP-c CTUh 4.5E-10 2.67E-12 4.72E-12 5.09E-14 1.11E-12 1.67E-11 -2.54E-13
HTP-nc CTUh 3.02E-08 1.31E-10 3.22E-10 3.52E-12 5.51E-11 1.85E-09 -9.74E-12
SQP SQP 2.03E+01 1.2E-03 2.04E-01 2.28E-05 4.98E-04 4.07E-02 -4.51E-03
PM = Potential incidence of disease due to PM emissions; IR = Potential Human exposure efficiency relative to U235; ETP-fw = Potential comparative
Toxic Unit for ecosystems; HTP-c = Potential comparative Toxic Unit for humans (cancerogenic); HTP-nc = Potential comparative Toxic Unit for humans
(not cancerogenic); SQP = Potential soil quality index
Disclaimer 1 – for the indicator 'Potential Human exposure efficiency relative to U235'. This impact category deals mainly with the
eventual impact of low-dose ionizing radiation on human health of the nuclear fuel cycle. It does not consider effects due to possible
nuclear accidents, occupational exposure nor due to radioactive waste disposal in underground facilities. Potential ionizing radiation
from the soil, from radon and from some construction materials is also not measured by this indicator.
Disclaimer 2 – for the indicators 'abiotic depletion potential for non-fossil resources', 'abiotic depletion potential for fossil resources',
'water (user) deprivation potential, deprivation-weighted water consumption', 'potential comparative toxic unit for ecosystems', 'potential
comparative toxic unit for humans – cancerogenic', 'Potential comparative toxic unit for humans - not cancerogenic', 'potential soil
quality index'. The results of this environmental impact indicator shall be used with care as the uncertainties on these results are high
or as there is limited experienced with the indicator. This EPD was created using a software tool. This EPD was created using a
software tool.
References
EN 15804 to-sustainability/
EN 15804:2012+A1:2013, Sustainability of construction works
— Environmental Product Declarations — Core rules for the LCA for Expert
product category of construction products. Life cycle assessment software (version 10), by Sphera
EN 15804 Solutions GmbH, Leinfelden-Echterdingen, 2022
EN 15804:2012+A2:2019+AC:2021, Sustainability of https://sphera.com/life-cycle-assessment-lca-software/
construction works — Environmental Product Declarations —
Core rules for the product category of construction products. Managed LCA Content
ISO 14025 Life cycle assessment database, by Sphera Solutions GmbH,
EN ISO 14025:2011, Environmental labels and declarations — Leinfelden-Echterdingen, 2022
Type III environmental declarations — Principles and https://sphera.com/life-cycle-assessment-lca-database/
procedures.
PCR Part A
PCR - Part A: Calculation rules for the Life Cycle Assessment
Further References and Requirements on the Background Report, version 1.3,
Institut Bauen und Umwelt e.V., 08-2021.
IBU 2021 PCR Part B
Institut Bauen und Umwelt e.V.: General Instructions for the PCR – Part B:Requirements on the EPD for Concrete
EPD programme of Institut Bauen und Umwelt e.V., Version admixtures, Institut Bauen und Umwelt e.V., 04-2023.
2.0, Berlin: Institut Bauen und Umwelt e.V., 2021 www.ibu-
epd.com ΕΝ934-2:2009+Α1:2012Admixtures for concrete, mortar and
grout - Part 2: Concrete admixtures - Definitions, requirements,
LCA Calculator conformity, marking and labelling.
LCA Calculator software (version 6). Visualize, Improve and
Report on Product Sustainability. https://sphera.com/your-path-
5 Environmental Product Declaration - Sika Hellas ABEE - SikaTard®-930
Publisher
Institut Bauen und Umwelt e.V. +49 (0)30 3087748- 0
Hegelplatz 1 info@ibu-epd.com
10117 Berlin www.ibu-epd.com
Germany
Programme holder
Institut Bauen und Umwelt e.V. +49 (0)30 3087748- 0
Hegelplatz 1 info@ibu-epd.com
10117 Berlin www.ibu-epd.com
Germany
Author of the Life Cycle Assessment
Sphera GmbH +49711341817-0
Hauptstrasse 111 info@sphera.com
70771 Echterdingen-Leinfelden www.sphera.com
Germany
Owner of the Declaration
SIKA HELLAS ABEE 6979970408
PROTOMAGIAS STR. 15 zacharopoulou.aggeliki@gr.sika.com
14568 athens https://grc.sika.com/
Greece
6 Environmental Product Declaration - Sika Hellas ABEE - SikaTard®-930
