ENVIRONMENTAL PRODUCT DECLARATION
as per ISO 14025 and EN 15804+A2
Owner of the Declaration Sika Australia Pty Ltd
Publisher Institut Bauen und Umwelt e.V. (IBU)
Programme holder Institut Bauen und Umwelt e.V. (IBU)
Declaration number EPD-SIK-20240176-CBA2-EN
Issue date 22/07/2024
Valid to 21/07/2029
Sika® ViscoCrete® PC HRF-2
Sika Australia Pty Ltd
www.ibu-epd.com | https://epd-online.com
General Information
Sika Australia Pty Ltd Sika® ViscoCrete® PC HRF-2
Programme holder Owner of the declaration
IBU – Institut Bauen und Umwelt e.V. Sika Australia Pty Ltd
Hegelplatz 1 Elizabeth Street 55
10117 Berlin 2164 Wetherill Park, NSW
Germany Australia
Declaration number Declared product / declared unit
EPD-SIK-20240176-CBA2-EN 1 kg of Sika® ViscoCrete® PC HRF-2 with a density of 1.08 kg/l.
This declaration is based on the product category rules: Scope:
Concrete admixtures, 01/08/2021 This verified EPD relates to 1kg of Sika® ViscoCrete® PC HRF-2. It is
(PCR checked and approved by the SVR) manufactured at the plants of Sika Australia Pty Ltd in Wetherill Park (NSW
2164), Keysborough (VIC 3173), Pinkenba (QLD 4008), and Bibra Lake
(WA 6163) in Australia. The production and transport data are
Issue date representative for the period from July 2022 to June 2023. The results in
this EPD are calculated using an LCA-tool verified by IBU in 2023.
22/07/2024
The owner of the declaration shall be liable for the underlying information
and evidence; the IBU shall not be liable with respect to manufacturer
Valid to
information, life cycle assessment data and evidences.
21/07/2029
The EPD was created according to the specifications of EN 15804+A2. In
the following, the standard will be simplified as EN 15804.
Verification
The standard EN 15804 serves as the core PCR
Independent verification of the declaration and data according to ISO
14025:2011
internally X externally
Dipl.-Ing. Hans Peters
(Chairman of Institut Bauen und Umwelt e.V.)
Florian Pronold Matthias Schulz,
(Managing Director Institut Bauen und Umwelt e.V.) (Independent verifier)
1 Environmental Product Declaration - Sika Australia Pty Ltd - Sika® ViscoCrete® PC HRF-2
Product
Additional technical data are not relevant for this product.
Product description/Product definition
Sika® ViscoCrete® PC HRF-2 is produced utilising Sika's Base materials/Ancillary materials
polycarboxylate technology. The product is a liquid agent that is The raw materials and additives of Sika® ViscoCrete® PC
introduced into concrete while it is being mixed. Depending on HRF-2 can be given as follows:
application, the typical dosage can range from 200 ml to 1000 Name Value Unit
ml per 100 kg of total cementitious materials. Optimum dosage
Polycarboxylate(s) (*) 40–70 %
should be determined by site trials with the particular concrete
Water 30–50 %
mix design and materials. Users shall refer to the most recent
Product Data Sheet for more information and advice. Additives < 10 %
(*) Solid content of 50%
Sika® ViscoCrete® PC HRF-2 is accompanied by a declaration
of performance, which conforms to the specifications outlined in
With respect to international and local regulations:
Australian Standard AS 1478.1-2000, type HWR. The product
• This product/article/at least one partial article contains
is designed to achieve enhanced workability and high strength
substances listed in the 'Candidate List of Substances of
characteristics of concrete. It can be used for most concrete
Very High Concern (SVHC) for Authorisation' (date:
applications including but not limited to high strength, high
30/05/2024) exceeding 0.1 percentage by mass: No.
performance, self-compacting, precast, pumped, and pre-
• Biocide products were added to this construction
stressed concrete.
product or it has been treated with biocide products (this
Application then concerns a treated product as defined by the (EU)
Sika® ViscoCrete® PC HRF-2 is used as a constituent material Ordinance on Biocide Products No. 528/2012): Yes. The
to produce concrete. It can be used in combination with other active substance in the biocide is octhilinone. The
Sika admixtures. All admixtures must be added separately and biocide was used as an in-can preservative.
trials are recommended before use. It can also be successfully • Any applicable prohibition, authorisation and restricted
used in mix designs utilising supplementary cementitious use requirements for this product, including for
materials. carcinogens referred to in Schedule 10 of the Australian
Model Work Health and Safety Regulations (WHS): No.
Technical Data
Sika® ViscoCrete® PC HRF-2 meets the requirements of AS
Reference service life
1478.1-2000, type HWR.
The durability of concrete admixtures is normally at least as
Constructional data
long as the lifetime of the building in which it is used. The
Name Value Unit experimental data show that the reference life is greater than
pH of admixture (AS 1478.1) 4.5–6.5 - 50 years. The documentation of the Reference service life is
1.06– not required for the EPDs calculated using the EPD tool from
Relative density of admixture (AS 1478.1) kg/l
1.10 Sika since the entire life cycle is not declared. Only modules
A1-A3, A4, A5, C1, C2, C4, and D are considered.
32.5–
Non-volatile content of admixture (AS 1478.1) %
36.5
Chloride content of admixture (AS 1478.1) ≤ 1.5 g/l
Water content of concrete as % of control (AS
≤ 85 %
1478.1)
Intial setting time of concrete, deviation from
-1 to +1 hour
control (AS 1012.18)
Final setting time of concrete, deviation from
-1 to +1 hour
control (AS 1012.18)
Compressive strength of concrete as % of
≥ 130 %
control at 1 day (AS 1012.9)
Compressive strength of concrete as % of
≥ 125 %
control at 3 days (AS 1012.9)
Compressive strength of concrete as % of
≥ 120 %
control at 7 days (AS 1012.9)
Compressive strength of concrete as % of
≥ 115 %
control at 28 days (AS 1012.9)
Compressive strength of concrete as % of
≥ 110 %
control at 90 days (AS 1012.9)
LCA: Calculation rules
Declared unit and mass reference
Declared Unit
The EPD refers to the declared unit of 1kg of concrete Name Value Unit
admixture applied into the building with a density of 1.08 g/ml in Declared unit 1 kg
accordance with IBU PCR 04-2023 Part B for concrete Gross density 1080 kg/m3
admixtures.
2 Environmental Product Declaration - Sika Australia Pty Ltd - Sika® ViscoCrete® PC HRF-2
Other declared units are allowed if the conversion is shown module) where all the impacts related to the transport
transparently. processes are considered.
One scenario is considered for the final treatment of the waste:
System boundary
• 100% disposal (C4), modelled by landfill process where
Declaration type with respect to life cycle stages covered
admixtures end their life cycle.
according to clause 5.2 EN 15804+A2 is cradle to gate with
Module D accounts for benefits that are beyond the defined
modules C1–C4 and module D (A1–A3, A4, A5, C and D).
system boundaries. Credits are generated during the
Modules taken into account:
incineration of the installation scrap in module A5.
• A1 Production of preliminary products
• A2 Transport to the plant
• A3 Production including provision of energy, production Geographic Representativeness
of auxiliaries and consumables and waste treatment Land or region, in which the declared product system is
• A4 Transport from the construction site to the installation manufactured, used or handled at the end of the product´s
site lifespan: Australia
• A5 Installation, admixtures applied into the building
during A5 phase operations. At this stage, an impact of
Comparability
the production and treatment of installation residue
equal to 1% of the product is considered. Basically, a comparison or an evaluation of EPD data is only
• C1-C2-C4-D possible if all the data sets to be compared were created
The building deconstruction (demolition process) takes place in according to EN 15804 and the building context, respectively
C1 module which considers energy production and the product-specific characteristics of performance, are taken
consumption in terms of diesel and all the emissions connected into account. Sphera LCA for Expert software (former GaBi)
with the fuel-burning process. After the demolition, the (version 10) and Managed LCA Content (2022.2) have been
admixture is transported to the end-of-life processing (C2 used.
LCA: Scenarios and additional technical information
Assembly (A5)
Characteristic product properties of biogenic carbon
The product contains small amounts of a substance with Name Value Unit
renewable primary energy resources used as raw materials Material loss 0.01 kg
(PERM), however, this is not calculated in the LCA tool and a Other resources - kg
PERM value of 0 in A1-A3 is declared.
Material loss regards the amount of product not used during the
application phase into the building. This amount is 1% of the
Information on describing the biogenic carbon content at product, impacts related to the production of this part are
factory gate charged to the A5 module. This percentage is considered as
Name Value Unit waste to incineration since the product has a calorific value and
kg impacts of its end of life have been considered in the LCA
Biogenic carbon content in product 0.00001 C model and declared in A5.
Biogenic carbon content in accompanying kg
-
packaging C End of life (C1-C4)
C1: This module considers the use of machinery (7.5E-5 kg of
Note: 1 kg of biogenic carbon is equivalent to 44/12 kg of CO .
2 diesel for kg handled) to dismantle the product to enable its
subsequent transport.
C2: The concrete demolition waste is transported from the
building site to a treatment plant or disposal site by truck and
Transport from the gate to the site (A4) an average distance of 50 km is considered.
Name Value Unit C4: The results for the end-of-life are declared for one scenario:
Transport distance 76 km Name Value Unit
Gross weight 34–40 t Landfill percentage 100 %
Payload capacity 27 t Material to landfill 1 kg
3 Environmental Product Declaration - Sika Australia Pty Ltd - Sika® ViscoCrete® PC HRF-2
LCA: Results
DESCRIPTION OF THE SYSTEM BOUNDARY (X = INCLUDED IN LCA; MND = MODULE OR INDICATOR NOT DECLARED; MNR
= MODULE NOT RELEVANT)
Benefits and
Construction loads beyond
Product stage Use stage End of life stage
process stage the system
boundaries
la ire ta m w a Ry lp p u s tro p s n a rT g n iru tc a fu n a M e h t m o rf tro p s n a rTe tis e h t o t e ta g y lb m e s s A e s U e c n a n e tn ia M ria p e R tn e m e c a lp e R tn e m h s ib ru fe R y g re n e la n o ita re p Oe s u re ta w la n o ita re p Oe s u n o itc u rts n o c -e Dn o itilo m e d tro p s n a rT g n is s e c o rp e ts a W la s o p s iD -e s u e R-y re v o c e R-g n ilc y c e Rla itn e to p
A1 A2 A3 A4 A5 B1 B2 B3 B4 B5 B6 B7 C1 C2 C3 C4 D
X X X X X MND MND MNR MNR MNR MND MND X X MND X X
RESULTS OF THE LCA - ENVIRONMENTAL IMPACT according to EN 15804+A2: 1 kg Sika® ViscoCrete® PC HRF-2
Parameter Unit A1-A3 A4 A5 C1 C2 C4 D
GWP-total kg CO 2 eq 9.01E-01 3.81E-03 2.27E-02 2.82E-04 6.27E-03 4.33E-02 -4.83E-03
GWP-fossil kg CO 2 eq 9.02E-01 3.65E-03 1.7E-02 2.7E-04 6E-03 4.29E-02 -4.83E-03
GWP-biogenic kg CO 2 eq -2.02E-03 1.62E-04 5.66E-03 1.21E-05 2.65E-04 4.41E-04 9.05E-07
GWP-luluc kg CO 2 eq 1.02E-04 9.53E-08 1.85E-06 7.16E-09 1.56E-07 1.53E-05 -2.34E-06
ODP kg CFC11 eq 1.49E-12 3.58E-16 2.06E-14 2.69E-17 5.88E-16 6.67E-14 -1.67E-14
AP mol H+ eq 3.86E-03 1.12E-05 1.22E-04 3.66E-06 2E-05 2.12E-04 -1.6E-05
EP-freshwater kg P eq 7.78E-06 4.61E-10 4.73E-08 3.47E-11 7.56E-10 1.33E-07 -1.68E-09
EP-marine kg N eq 1.04E-03 4.98E-06 1.96E-05 1.65E-06 9.02E-06 5.73E-05 -3.5E-06
EP-terrestrial mol N eq 1.13E-02 5.47E-05 2.5E-04 1.81E-05 9.93E-05 6.3E-04 -3.81E-05
kg NMVOC
POCP 3.14E-03 1.01E-05 6.52E-05 4.96E-06 1.8E-05 1.57E-04 -1.04E-05
eq
ADPE kg Sb eq 4.22E-07 1.48E-10 2.72E-09 1.11E-11 2.43E-10 1.14E-08 -2.86E-10
ADPF MJ 2.17E+01 5.05E-02 3.17E-01 3.8E-03 8.29E-02 6.22E-01 -5.14E-02
m3 world eq
WDP 2.77E-01 3.11E-05 4.02E-03 2.34E-06 5.1E-05 2.6E-03 -1.38E-03
deprived
GWP = Global warming potential; ODP = Depletion potential of the stratospheric ozone layer; AP = Acidification potential of land and water; EP =
Eutrophication potential; POCP = Formation potential of tropospheric ozone photochemical oxidants; ADPE = Abiotic depletion potential for non-fossil
resources; ADPF = Abiotic depletion potential for fossil resources; WDP = Water (user) deprivation potential)
RESULTS OF THE LCA - INDICATORS TO DESCRIBE RESOURCE USE according to EN 15804+A2: 1 kg Sika® ViscoCrete® PC
HRF-2
Parameter Unit A1-A3 A4 A5 C1 C2 C4 D
PERE MJ 1.33E+00 2.73E-04 1.7E-02 2.06E-05 4.49E-04 6.01E-02 -1.18E-02
PERM MJ 0 0 0 0 0 0 0
PERT MJ 1.33E+00 2.73E-04 1.7E-02 2.06E-05 4.49E-04 6.01E-02 -1.18E-02
PENRE MJ 1.71E+01 5.06E-02 3.21E-01 3.8E-03 8.3E-02 6.41E-01 -5.14E-02
PENRM MJ 4.82E+00 0 -3.68E-03 0 0 0 0
PENRT MJ 2.2E+01 5.06E-02 3.18E-01 3.8E-03 8.3E-02 6.41E-01 -5.14E-02
SM kg 0 0 0 0 0 0 0
RSF MJ 0 0 0 0 0 0 0
NRSF MJ 0 0 0 0 0 0 0
FW m3 9.68E-03 7.84E-07 1.18E-04 5.89E-08 1.29E-06 9.2E-05 -3.3E-05
PERE = Use of renewable primary energy excluding renewable primary energy resources used as raw materials; PERM = Use of renewable primary
energy resources used as raw materials; PERT = Total use of renewable primary energy resources; PENRE = Use of non-renewable primary energy
excluding non-renewable primary energy resources used as raw materials; PENRM = Use of non-renewable primary energy resources used as raw
materials; PENRT = Total use of non-renewable primary energy resources; SM = Use of secondary material; RSF = Use of renewable secondary fuels;
NRSF = Use of non-renewable secondary fuels; FW = Use of net fresh water
RESULTS OF THE LCA – WASTE CATEGORIES AND OUTPUT FLOWS according to EN 15804+A2:
1 kg Sika® ViscoCrete® PC HRF-2
Parameter Unit A1-A3 A4 A5 C1 C2 C4 D
HWD kg 1.39E-09 1.27E-13 1.46E-11 9.52E-15 2.08E-13 2.4E-11 -4.8E-12
NHWD kg 5.43E-02 2.1E-06 1.96E-03 1.58E-07 3.44E-06 1E+00 -2.19E-05
RWD kg 2.67E-04 2.85E-08 2.5E-06 2.14E-09 4.67E-08 5.63E-06 -9.94E-07
CRU kg 0 0 0 0 0 0 0
MFR kg 0 0 0 0 0 0 0
MER kg 0 0 0 0 0 0 0
EEE MJ 0 0 2E-02 0 0 0 0
EET MJ 0 0 4.18E-03 0 0 0 0
4 Environmental Product Declaration - Sika Australia Pty Ltd - Sika® ViscoCrete® PC HRF-2
HWD = Hazardous waste disposed; NHWD = Non-hazardous waste disposed; RWD = Radioactive waste disposed; CRU = Components for re-use;
MFR = Materials for recycling; MER = Materials for energy recovery; EEE = Exported electrical energy; EET = Exported thermal energy
RESULTS OF THE LCA – additional impact categories according to EN 15804+A2-optional:
1 kg Sika® ViscoCrete® PC HRF-2
Parameter Unit A1-A3 A4 A5 C1 C2 C4 D
Disease
PM 4.79E-08 6.19E-11 1.1E-09 1.93E-10 1.08E-10 2.21E-09 -2.19E-10
incidence
IR kBq U235 eq 2.73E-02 1.89E-06 3.27E-04 1.42E-07 3.1E-06 5.17E-04 -6.21E-05
ETP-fw CTUe 1.08E+01 5.98E-02 2.32E-01 4.5E-03 9.82E-02 3.47E-01 -9.38E-03
HTP-c CTUh 1.41E-09 9.6E-13 6.71E-12 7.22E-14 1.58E-12 3.35E-11 -8.96E-13
HTP-nc CTUh 1.51E-07 3.29E-11 3.65E-10 3.5E-12 5.47E-11 3.51E-09 -2.33E-11
SQP SQP 3.35E+00 1.49E-04 3.57E-02 1.12E-05 2.45E-04 7.32E-02 -5.09E-03
PM = Potential incidence of disease due to PM emissions; IR = Potential Human exposure efficiency relative to U235; ETP-fw = Potential comparative
Toxic Unit for ecosystems; HTP-c = Potential comparative Toxic Unit for humans (cancerogenic); HTP-nc = Potential comparative Toxic Unit for humans
(not cancerogenic); SQP = Potential soil quality index
Disclaimer 1 – for the indicator 'Potential Human exposure efficiency relative to U235'. This impact category deals mainly with the
eventual impact of low-dose ionizing radiation on human health of the nuclear fuel cycle. It does not consider effects due to possible
nuclear accidents, occupational exposure or radioactive waste disposal in underground facilities. Potential ionizing radiation from the
soil, radon and from some construction materials is also not measured by this indicator.
Disclaimer 2 – for the indicators 'abiotic depletion potential for non-fossil resources', 'abiotic depletion potential for fossil resources',
'water (user) deprivation potential, deprivation-weighted water consumption', 'potential comparative toxic unit for ecosystems', 'potential
comparative toxic unit for humans – cancerogenic', 'Potential comparative toxic unit for humans - not cancerogenic', 'potential soil
quality index'. The results of this environmental impact indicator shall be used with care as the uncertainties on these results are high
as there is limited experience with the indicator. This EPD was created using a software tool.
References
AS 1012.9:2014
Methods of testing concrete - Method 9: Determination of the Further References
compressive strength of concrete specimens
IBU General Instructions
AS 1012.18-1996 (R-2014) General Instructions for the EPD programme of Institut Bauen
Methods of testing concrete - Method 18: Determination of und Umwelt e.V., Version 2.1, Berlin: Institut Bauen und Umwelt
setting time of fresh concrete, mortar and grout by penetration e.V., 2022, www.ibu-epd.com
resistance
LCA Calculator
AS 1478.1-2000 LCA Calculator software (version 6), by Sphera Solutions
Chemical admixtures for concrete, mortar and grout - Part 1: GmbH, Leinfelden-Echterdingen, 2024
Admixtures for concrete
LCA for Expert
Candidate List of SVHC Life cycle assessment software (version 10), by Sphera
Candidate List of Substances of Very High Concern for Solutions GmbH, Leinfelden-Echterdingen, 2022,
Authorisation, European Chemicals Agency (ECHA), 2024, https://sphera.com/life-cycle-assessment-lca-software/
https://echa.europa.eu/candidate-list-table
Managed LCA Content
EN 15804:2012+A2:2019+AC:2021 Life Cycle Assessment databases, Sphera Solutions GmbH,
Sustainability of construction works — Environmental Product Leinfelden-Echterdingen, 2022, https://sphera.com/life-cycle-
Declarations — Core rules for the product category of assessment-lca-database/
construction products
PCR Part A
ISO 14025:2011 PCR - Part A: Calculation rules for the Life Cycle Assessment
Environmental labels and declarations — Type III and Requirements on the Background Report, version 1.3,
environmental declarations — Principles and procedures Institut Bauen und Umwelt e.V., 08-2021
Model WHS Regulations PCR Part B
Schedule 10 Prohibited carcinogens, restricted carcinogens PCR – Part B: Requirements on the EPD for Concrete
and restricted hazardous chemicals, Australian Model Work admixtures, Institut Bauen und Umwelt e.V., 04-2023
Health and Safety Regulations, 08-2023
5 Environmental Product Declaration - Sika Australia Pty Ltd - Sika® ViscoCrete® PC HRF-2
Publisher
Institut Bauen und Umwelt e.V. +49 (0)30 3087748- 0
Hegelplatz 1 info@ibu-epd.com
10117 Berlin www.ibu-epd.com
Germany
Programme holder
Institut Bauen und Umwelt e.V. +49 (0)30 3087748- 0
Hegelplatz 1 info@ibu-epd.com
10117 Berlin www.ibu-epd.com
Germany
Author of the Life Cycle Assessment
Sphera Solutions GmbH +49 (0)711 341817-0
Hauptstraße 111- 113 info@sphera.com
70771 Leinfelden-Echterdingen www.sphera.com
Germany
Owner of the Declaration
Sika Australia Pty Ltd +61 2 9725 1145
Elizabeth Street 55 sustainability@au.sika.com
2164 Wetherill Park, NSW aus.sika.com
Australia
6 Environmental Product Declaration - Sika Australia Pty Ltd - Sika® ViscoCrete® PC HRF-2
