ENVIRONMENTAL PRODUCT DECLARATION
as per ISO 14025 and EN 15804+A2
Owner of the Declaration Uzin Utz SE
Publisher Institut Bauen und Umwelt e.V. (IBU)
Programme holder Institut Bauen und Umwelt e.V. (IBU)
Declaration number EPD-UZI-20230497-IBC2-EN
Issue date 29.01.2024
Valid to 28.01.2029
Skirting Tapes
Sifloor AG
www.ibu-epd.com | https://epd-online.com
1. General Information
Sifloor AG Skirting Tapes
Programme holder Owner of the declaration
IBU – Institut Bauen und Umwelt e.V. Uzin Utz SE
Hegelplatz 1 Dieselstraße 3
10117 Berlin 89079 Ulm
Germany Germany
Declaration number Declared product / declared unit
EPD-UZI-20230497-IBC2-EN 1 m2 of: Skirting Tapes
This declaration is based on the product category rules: Scope:
Dispersion adhesives and primers for floor coverings, 01.08.2021 This Environmental Product Declaration is an average EPD for dry
(PCR checked and approved by the SVR) adhesives covering the products: UZIN Toptac, UZIN Goman, UZIN U-
Tack, UZIN Bullran, UZIN Remur, UZIN Linomur.
The data provided in this EPD refers to the arithmetic mean of the products
Issue date mentioned. All products covered by this EPD are manufactured at the
Sifloor AG plant in Sursee, Switzerland.
29.01.2024
The owner of the declaration shall be liable for the underlying information
and evidence; the IBU shall not be liable with respect to manufacturer
information, life cycle assessment data and evidences.
Valid to
28.01.2029 The EPD was created according to the specifications of EN 15804+A2. In
the following, the standard will be simplified as EN 15804.
Verification
The standard EN 15804 serves as the core PCR
Independent verification of the declaration and data according to ISO
14025:2011
internally X externally
Dipl.-Ing. Hans Peters
(Chairman of Institut Bauen und Umwelt e.V.)
Florian Pronold Matthias Schulz,
(Managing Director Institut Bauen und Umwelt e.V.) (Independent verifier)
1 Environmental Product Declaration - Sifloor AG - Skirting Tapes
2. Product
EC1 Plus according to the EMICODE requirements.
2.1 Product description/Product definition Furthermore, products are awarded with the Blue Angel (DE-UZ
This EPD comprises dry adhesives of the product category: 113) due to their low emissions.
Skirting -Tapes. All products considered here are based on the
switchTec dry adhesive technology. This is a technology for REACH regulation:
floor/socket bonding and fulfils the function of liquid adhesives
as an alternative. Does this product/article/at least one partial article contains
The following products can be assigned to this EPD: substances listed in the candidate list (date: 01.01.2024)
• UZIN Toptac exceeding 0.1 percentage by mass?
• UZIN Goman NO
• UZIN U-Tack
• UZIN Bullran Does this product/article/at least one partial article contains
• UZIN Remur other CMR substances in categories 1A or 1B which are not on
• UZIN Linomur the candidate list, exceeding 0.1 percentage by mass?
For the use and application of the product the respective NO
national provisions at the place of use apply, in Germany for
example the building codes of the federal states and the Were biocide products added to this construction product or
corresponding national specifications. has it been treated with biocide products (this then concerns a
treated product as defined by the (EU) Ordinance on Biocide
2.2 Application Products No. 528/2012)?
The different skirting tapes are specially adapted to different NO
substrates and coverings and are suitable for bonding of Information on hazardous substances (if any) contained in this
Skirting boards, strips, flutes and stair flooring. product can be found in the product specific Safety Data sheet.
The latest version is available at our Website:
2.3 Technical Data https://int.uzin.com/
The various foil tapes are specially adapted to different
substrates and floor coverings to comply with their
requirements. 2.6 Manufacture
The ingredients of the adhesive component are first added
Constructional data
together according to the corresponding formula and mixed
Name Value Unit
under continuous stirring. In two steps, the adhesive
Dimensional changes (in transverse direction) component is then first applied to the carrier material on one
acc. to ISO 22633 (Dispersion adhesives for side and dried in the oven. The process is then repeated for the
textile and elastic floor coverings, not applicable max. other side in a second step. Some substrates are such that the
<0.2%
for polyvinyl chloride floor coverings, rubber floor % adhesive component penetrates the substrate. In this case, one
coverings, smooth polyolefin floor coverings, coating cycle is sufficient and the second adhesive coating step
textile floor coverings) is omitted. In order to prevent the skirting tape from sticking
Dimensional changes acc. to ISO 22635 when it is rolled up, a protective paper (liner) is applied to one
(Dispersion adhesives for textile and elastic floor max. of the adhesive sides.
<0.2%
coverings, (not applicable for linoleum or textile %
2.7 Environment and health during manufacturing
floor coverings)
Apart from the standard precautions for occupational hygiene
Other constructional data are not relevant for this product.
and safety, there are no special protective precautions to be
observed during production.
Performance data of the product with respect to its
characteristics in accordance with the relevant technical 2.8 Product processing/Installation
provision (no CE-marking). Dry adhesives are applied by hand on appropriately prepared
substrates. To do so, the skirting tape is rolled out on the
2.4 Delivery status
substrate under pressure. To install the covering, the tapes are
The different products covered by this EPD are delivered in
first rolled out to an area to be installed and rubbed in
different packaging, depending of the size of the tape and the
thoroughly with a textile cork rubbing board. Then it is cut to
number of tapes contained in one packaging-box. Detailed
size with a hook knife. Afterwards, the protective paper on the
information can be found at our Website: https://int.uzin.com/
opposite side is peeled off, revealing a second adhesive side.
In the last step, the floor covering can be applied to the second
2.5 Base materials/Ancillary materials
adhesive side by applying pressure on it.
Dry adhesives in general consist of a carrier material with a
self-adhesive layer on both sides. On average, the skirting 2.9 Packaging
tapes covered by this EPD are composed of:
The skirting tape is packed in a cardboard packaging. Emptied
Name Value Unit cores and cardboard packaging are recyclable. The weight and
Synthetic polymer dispersion (solid content) 40 - 60 % shape of the packaging are different for the products
Water 20 - 35 % considered here. More details can be found under Section 2.4.
Additives 0-2 % 2.10 Condition of use
Liner (protective paper) 5 - 30 % The substantial composition during the use phase refers to the
Carrier material 0.5 - 10 % composition during the manufacturing. Compared to liquid
adhesives, dry adhesives do not harden through chemical
All products covered by this EPD are very low in volatile organic
reactions, but are permanently adhesive and do not dry out.
compound (VOC) emission. They are all certified as EMICODE
2 Environmental Product Declaration - Sifloor AG - Skirting Tapes
floor covering or insulation layers. Therefore, the fire resistance
class of the floor covering according to EN 13501 must be
2.11 Environment and health during use taken into account when assessing the fire behaviour. The fire
The products covered by this EPD have been awarded the classification of the floor covering to be installed will be
emission label EMICODE EC 1 PLUS "very low emission" and maintained when installed on switchTec dry adhesives.
the Blue Angel (DE-UZ 113). With the emission label, the dry Water
adhesives contribute to preserving a healthy indoor climate. Excessive amounts of water can damage the substrate or the
Details on the individual criteria of the EMICODE can be found floor covering. When the dry adhesive comes into contact with
under point 7 Requisite Evidence. water, the adhesive strength is weakened and returns to full
strength after the water has fully evaporated. No substances
All products covered by this EPD meet the highest DGNB are washed out that could be hazardous to water.
Quality Level 4. Furthermore, the products contribute to further
green building rating systems such as LEED and BREEAM. Mechanical destruction
Not of relevance.
2.12 Reference service life
The service life of dry adhesives depends on the service life of 2.14 Re-use phase
the floor covering. In turn, the service life of different coverings Since adhesive residues may remain on the covering and the
show a high variability (10-50 years according to the table substrate, it is usually disposed of together, respectively. The
"Service lives of components for life cycle assessment re-use of the tapes covered by this EPD is not possible.
according to Assessment System for Sustainable Building
(BNB)"; BBSR: Bundesinstitut für Bau-, Stadt- und 2.15 Disposal
Raumforschung; www.nachhaltigesbauen.de/baustoff- The EWC waste code in accordance with the European Waste
undgebaeudedaten/nutzungsdauern-von-bauteilen.html)) Catalogue / List of Waste Ordinance for cured dispersion waste
Therefore, the specification of a reference service life according bears the EWC waste code 080410 (adhesive and sealing
to ISO 15686 is not possible. compound waste). Material residues can be disposed of as
household waste.
2.13 Extraordinary effects
Fire 2.16 Further information
There are no normative requirements for fire protection for this Product and safety data sheet, EMICODE EC 1 PLUS and Blue
product group. The fire behaviour of the floor construction is Angel certificate, general building authority approval and further
primarily determined by the type and nature of the installed information at https://int.uzin.com/.
3. LCA: Calculation rules
3.1 Declared Unit 3.2 System boundary
This declaration is an average EPD and refers to 1 m2 of the Type of EPD: Cradle to gate with options, modules C1–C4, and
skirting tapes UZIN Toptac, UZIN Goman, UZIN U-Tack, UZIN module D (A1–A3 + C + D and additional modules). The
Bullran, UZIN Remur, UZIN Linomur, manufactured by additional modules are A4 and A5. The underlying LCA
SIFLOOR AG at the Sursee plant. All values stated in this EPD addresses all life cycle stages of the average product. The
represent the arithmetic mean of the individual values of the other life cycle stages are not relevant for the product class and
products. The products mentioned are manufactured at the no environmental impacts occur in these. The following
same plant and fulfil the same or a comparable function; other activities are covered by the relevant modules:
life cycle phases are the same, such as production. The • A1: Production of raw and auxiliary materials
declared unit of 1 m2 was chosen as the operating data is • A2: Transport of raw and auxiliary materials to the plant
recorded either per linear metre [m] or per square metre [m2] • A3: Production in the plant (incl. provision of energy and
and the sales unit is also given in m2. Using the conversion waste treatment) and the manufacture of the packaging
factor of the average mass per square metre, the data given • A4: Transport of the packed product to the construction
can be related to 1 kg. site
• A5: Installation of the product and disposal of the
packaging and waste produced during installation
Declared unit and mass reference
(including the protective paper)
Name Value Unit
• C1: Manual removal of the product
Declared Unit 1 m2 • C2: Transport for disposal
Gross density 1 - 1.5 kg/m3 • C3: As a worst-case scenario thermal treatment of the
product in an incineration plant is modelled as end-of-
Grammage (average over all products
0,462 kg/m2 life scenario
considered)
• C4: Not relevant because the product is incinerated
Layer thickness (average over all products
0,0004 m (respective impacts declared in C3)
considered)
• D: Credits resulting from thermal utilisation of the
The representativeness of the average LCA values is rated as product and packaging waste
good. Comparability with regard to temporal, geographical and
technological factors is ensured by the fact that all the products For the environmental impact, the use of green electricity was
considered here were manufactured in the same plant using calculated taking into account the residual electricity mix for the
the same machinery, while the same reference year was remaining electricity. The proportion of the on-site electricity
utilised. Differences may arise in the exact composition of the demand covered by green electricity in the total on-site
applied adhesive and its coating thickness, as well as the electricity demand is 100 %.
substrate material used.
Further information regarding the variability of specific impact
indicators is given in Chapter 6.
3 Environmental Product Declaration - Sifloor AG - Skirting Tapes
3.3 Estimates and assumptions 3.6 Data quality
No material loss was assumed in module A5 (installation), as The data quality can be classified as good. The plant-specific
this is strongly dependent on the application procedure. In data refer to the year 2022. All remaining data originate from
order to determine the environmental burdens caused by the the above-mentioned database, the contents of which are
compensation of the additional material effort due to the regularly reviewed to ensure their currency. Thus, the data used
material loss, the following scheme can be used: The material for the life cycle assessment are representative. For some input
loss expressed as a percentage [%] is multiplied by the materials, proxy datasets had to be used. All background
indicator values from modules A1-A4 and C3 and added to datasets used are less than 10 years old. Data sets are
module A5. A subtraction of the indicator values from modules complete and comply with the system boundaries and the cut-
A1-A4 and C3 is not necessary, as only the additional material off rules for inputs and outputs. The data quality thus meets the
effort to compensate for the material loss is considered. As end- requirements of PCR Part A.
of-life assumption for the packaging and the product, a 100 %
thermal treatment scenario was chosen, respectively. 3.7 Period under review
The year 2022 is used as the reference year.
Since different packaging is used by the products covered in
3.8 Geographic Representativeness
this EPD, as a worst-case assumption always the packaging
with the worst packaging weight to product weight ratio was Land or region, in which the declared product system is
declared. manufactured, used or handled at the end of the product´s
lifespan: Europe
3.4 Cut-off criteria
The common rules according to ISO 14044 were applied as
3.9 Allocation
cut-off criteria. These apply to the entire product system as well
Site-specific operating data was distributed to the different
as to individual process modules and take into account mass,
products according to the machine utilisation. The loads from
energy and environmental relevance. All inputs were included
thermal utilisation of:
in the LCA that are more than 1 % with regard to the total
impact of an impact category. Overall, no more than 5 % of the
3.10 Comparability
flows were neglected with regard to the cut-off criteria.
Basically, a comparison or an evaluation of EPD data is only
3.5 Background data possible if all the data sets to be compared were created
according to EN 15804 and the building context, respectively
Factory-specific data was used for the production processes.
the product-specific characteristics of performance, are taken
For all other life cycle phases, data sets from Sphera Managed
into account. The background database is used from Sphera
LCA Content (Content Version 2023.2) were used. The LCA
Managed LCA Content. In this EPD, dry adhesives are
model was created in the software LCA for Experts (Version 10)
considered. These differ from liquid dispersion adhesives in
(former GaBi).
their specific characteristics of performance and response to
(punctual) stresses, so a direct comparison is not possible.
4. LCA: Scenarios and additional technical information
Name Value Unit
Characteristic product properties of biogenic carbon
Transport distance (Stage 1) 450 km
Biogenic carbon content at the gate:
Gross weight (Stage 1) 34 - 40 t
Note: 1 kg of biogenic carbon is equivalent to 44/12 kg of CO2. Payload capacity (Stage 1) 27 t
Utilisation by mass (Stage 1) 0.61 -
Biogenic carbon in the product is only contained in the ------------------------------- ----------- ----------- -----
protective paper used, which reaches the end of its waste
Transport distance (Stage 2) 50 km
properties in A5 and is therefore fully emitted and booked out in
Gross weight (Stage 2) 7.5 - 12 t
A5 and not in C3.
Payload capacity (Stage 2) 5 t
Information on describing the biogenic carbon content at
Utilisation by mass (Stage 2) 0.61 -
factory gate
Name Value Unit Installation into the building (A5)
Biogenic carbon content in product (arithmetic 3.10E- kg Name ValueUnit
mean) 02 C
Auxiliary - kg
Biogenic carbon content in accompanying 1.89E- kg
Water consumption - m3
packaging 02 C
Other resources - kg
Electricity consumption - kWh
In the following, the technical scenario information is presented,
Other energy carriers - MJ
which enables a better understanding of the declared modules.
Material loss - kg
Transport to the building site (A4)
Output substances following waste treatment on
The transport was divided into two phases, which best 0.09 kg
site
correspond to the actual situation. In the first stage, the product
is transported to a wholesaler by a large truck. The second Dust in the air - kg
stage represents the transport from the wholesaler to the VOC in the air - kg
construction site, which is mostly done by the craftsman with a
No material loss was assumed in module A5 (installation), as
small truck.
this is strongly dependent on the application procedure. In
order to determine the environmental burdens caused by the
4 Environmental Product Declaration - Sifloor AG - Skirting Tapes
compensation of the additional material effort due to the The difference in mass between the product shipped and the
material loss, the following scheme can be used: The material product installed and thus to be disposed of in C3 differs due to
loss expressed as a percentage [%] is multiplied by the the protective paper which is removed during installation. The
indicator values from modules A1-A4 and C3 and added to waste treatment of the protective paper is declared in module
module A5. A subtraction of the indicator values from modules A5.
A1-A4 and C3 is not necessary, as only the additional material
effort to compensate for the material loss is considered.
The protective paper, attached to the product is disposed of
during the installation phase. Thermal treatment was assumed
as a worst-case scenario.
End of life (C1-C4)
Name ValueUnit
Collected as mixed construction waste (arithmetic
0.372 kg
mean)
Reuse - kg
Recycling - kg
Energy recovery 100 %
Landfilling 0 %
5 Environmental Product Declaration - Sifloor AG - Skirting Tapes
5. LCA: Results
DESCRIPTION OF THE SYSTEM BOUNDARY (X = INCLUDED IN LCA; MND = MODULE OR INDICATOR NOT DECLARED; MNR
= MODULE NOT RELEVANT)
Benefits and
Construction loads beyond
Product stage Use stage End of life stage
process stage the system
boundaries
la ire ta m w a Ry lp p u s tro p s n a rT g n iru tc a fu n a M e h t m o rf tro p s n a rTe tis e h t o t e ta g y lb m e s s A e s U e c n a n e tn ia M ria p e R tn e m e c a lp e R tn e m h s ib ru fe R y g re n e la n o ita re p Oe s u re ta w la n o ita re p Oe s u n o itc u rts n o c -e Dn o itilo m e d tro p s n a rT g n is s e c o rp e ts a W la s o p s iD -e s u e R-y re v o c e R-g n ilc y c e Rla itn e to p
A1 A2 A3 A4 A5 B1 B2 B3 B4 B5 B6 B7 C1 C2 C3 C4 D
X X X X X MND MND MNR MNR MNR MND MND X X X MND X
RESULTS OF THE LCA - ENVIRONMENTAL IMPACT according to EN 15804+A2: 1 m^2 Skirting Tape
Parameter Unit A1-A3 A4 A5 C1 C2 C3 D
GWP-total kg CO 2 eq 1.53E+00 2.07E-02 1.94E-01 0 8.08E-04 4.7E-01 -1.61E-01
GWP-fossil kg CO 2 eq 1.7E+00 2.05E-02 1.18E-02 0 7.98E-04 3.52E-01 -1.6E-01
GWP-biogenic kg CO 2 eq -1.97E-01 4.77E-05 1.83E-01 0 1.85E-06 1.18E-01 -7.21E-04
GWP-luluc kg CO 2 eq 2.12E-02 1.93E-04 3.63E-06 0 7.5E-06 9.73E-06 -1.03E-05
ODP kg CFC11 eq 1.92E-08 1.82E-15 2.85E-14 0 7.09E-17 8.55E-14 -1.23E-12
AP mol H+ eq 4.48E-03 7.22E-05 7.76E-05 0 2.78E-06 2.46E-04 -1.98E-04
EP-freshwater kg P eq 8.94E-06 7.59E-08 1.44E-08 0 2.95E-09 4.75E-08 -2.54E-07
EP-marine kg N eq 1.5E-03 3.33E-05 2.98E-05 0 1.28E-06 9.55E-05 -5.81E-05
EP-terrestrial mol N eq 1.38E-02 3.74E-04 3.46E-04 0 1.44E-05 1.09E-03 -6.23E-04
kg NMVOC
POCP 4.01E-03 6.52E-05 7.79E-05 0 2.51E-06 2.49E-04 -1.62E-04
eq
ADPE kg Sb eq 3.35E-06 1.35E-09 2.56E-10 0 5.26E-11 7.38E-10 -1.13E-08
ADPF MJ 4.02E+01 2.83E-01 7.65E-02 0 1.1E-02 2.27E-01 -2.95E+00
m3 world eq
WDP 2.74E-01 2.4E-04 2.2E-02 0 9.33E-06 5.87E-02 -1.49E-02
deprived
GWP = Global warming potential; ODP = Depletion potential of the stratospheric ozone layer; AP = Acidification potential of land and water; EP =
Eutrophication potential; POCP = Formation potential of tropospheric ozone photochemical oxidants; ADPE = Abiotic depletion potential for non-fossil
resources; ADPF = Abiotic depletion potential for fossil resources; WDP = Water (user) deprivation potential)
RESULTS OF THE LCA - INDICATORS TO DESCRIBE RESOURCE USE according to EN 15804+A2: 1 m^2 Skirting Tape
Parameter Unit A1-A3 A4 A5 C1 C2 C3 D
PERE MJ 6.88E+00 2E-02 1.76E+00 0 7.79E-04 4.58E-02 -8.42E-01
PERM MJ 1.74E+00 0 -1.74E+00 0 0 0 0
PERT MJ 8.62E+00 2E-02 2E-02 0 7.79E-04 4.58E-02 -8.42E-01
PENRE MJ 3.09E+01 2.84E-01 3.86E-01 0 1.1E-02 9.29E+00 -2.95E+00
PENRM MJ 9.37E+00 0 -3.09E-01 0 0 -9.06E+00 0
PENRT MJ 4.04E+01 2.84E-01 7.7E-02 0 1.1E-02 2.3E-01 -2.95E+00
SM kg 0 0 0 0 0 0 0
RSF MJ 0 0 0 0 0 0 0
NRSF MJ 0 0 0 0 0 0 0
FW m3 9.99E-03 2.21E-05 5.18E-04 0 8.59E-07 1.39E-03 -6.82E-04
PERE = Use of renewable primary energy excluding renewable primary energy resources used as raw materials; PERM = Use of renewable primary
energy resources used as raw materials; PERT = Total use of renewable primary energy resources; PENRE = Use of non-renewable primary energy
excluding non-renewable primary energy resources used as raw materials; PENRM = Use of non-renewable primary energy resources used as raw
materials; PENRT = Total use of non-renewable primary energy resources; SM = Use of secondary material; RSF = Use of renewable secondary fuels;
NRSF = Use of non-renewable secondary fuels; FW = Use of net fresh water
RESULTS OF THE LCA – WASTE CATEGORIES AND OUTPUT FLOWS according to EN 15804+A2:
1 m^2 Skirting Tape
Parameter Unit A1-A3 A4 A5 C1 C2 C3 D
HWD kg 1.34E-04 1.05E-12 2.58E-12 0 4.08E-14 8E-12 -1.63E-10
NHWD kg 6.12E-02 4.09E-05 1.78E-02 0 1.59E-06 6.43E-02 -1.44E-03
RWD kg 6.26E-04 3.67E-07 3.45E-06 0 1.43E-08 9.9E-06 -2.23E-04
CRU kg 0 0 0 0 0 0 0
MFR kg 0 0 0 0 0 0 0
MER kg 0 0 0 0 0 0 0
EEE MJ 0 0 2.2E-01 0 0 5.23E-01 0
EET MJ 0 0 4.07E-01 0 0 9.81E-01 0
HWD = Hazardous waste disposed; NHWD = Non-hazardous waste disposed; RWD = Radioactive waste disposed; CRU = Components for re-use;
MFR = Materials for recycling; MER = Materials for energy recovery; EEE = Exported electrical energy; EET = Exported thermal energy
6 Environmental Product Declaration - Sifloor AG - Skirting Tapes
RESULTS OF THE LCA – additional impact categories according to EN 15804+A2-optional:
1 m^2 Skirting Tape
Parameter Unit A1-A3 A4 A5 C1 C2 C3 D
Disease
PM ND ND ND ND ND ND ND
incidence
IR kBq U235 eq ND ND ND ND ND ND ND
ETP-fw CTUe ND ND ND ND ND ND ND
HTP-c CTUh ND ND ND ND ND ND ND
HTP-nc CTUh ND ND ND ND ND ND ND
SQP SQP ND ND ND ND ND ND ND
PM = Potential incidence of disease due to PM emissions; IR = Potential Human exposure efficiency relative to U235; ETP-fw = Potential comparative
Toxic Unit for ecosystems; HTP-c = Potential comparative Toxic Unit for humans (cancerogenic); HTP-nc = Potential comparative Toxic Unit for humans
(not cancerogenic); SQP = Potential soil quality index
Disclaimer 1 – for the indicator 'Potential Human exposure efficiency relative to U235'. This impact category deals mainly with the
eventual impact of low-dose ionizing radiation on human health of the nuclear fuel cycle. It does not consider effects due to possible
nuclear accidents, occupational exposure or radioactive waste disposal in underground facilities. Potential ionizing radiation from the
soil, radon and from some construction materials is also not measured
by this indicator. Disclaimer 2 – for the indicators 'abiotic depletion potential for non-fossil resources', 'abiotic depletion potential for
fossil resources', 'water (user) deprivation potential, deprivation-weighted water consumption', 'potential comparative toxic unit for
ecosystems', 'potential comparative toxic unit for humans – cancerogenic', 'Potential comparative toxic unit for humans - not
cancerogenic', 'potential soil quality index'. The results of this environmental impact indicator shall be used with care as the
uncertainties on these results are high as there is limited experience with the indicator
Disclaimer 3: Additional environmental impact indicators (EN 15804, Table 4) are not declared in the EPD. The results of these
environmental impact indicators should be used with caution as the uncertainties in these results are high and there is limited
experience with the indicators (see ILCD classification in EN 15804, Table 5). For this reason, the results based on these indicators are
not reported.
6. LCA: Interpretation
The coefficient of variation is a measure of the relative scatter.
It indicates what percentage of the average the standard
deviation is. It is therefore the percentage ratio of the standard
deviation to the arithmetic mean. It is used to make it easier to
compare the spread of different distributions. The spread of the
impact indicators is generally moderate and at about the same
level for all indicators.
Alongside the coefficient of variation, the maximum deviation of
individual products' impact from the average value for specific
impact indicators was also analysed (see table below). These
show that some impact indicators such as Ozone Depletion
react sensitively to individual substances contained, resulting in
a high deviation. In general, however, the results are in the
same order of magnitude, which indicates a appropriate
grouping.
The dominance analysis of the impact assessment indicators
shows a large contribution from the manufacturing phase (A1-
A3). A large proportion of the environmental impact stems from
the raw materials used (A1), with the synthetic polymer
dispersions making the highest contributions (with regard to the
impact indicator Climate Change - total, an average of 95% of
the impact in A1 is attributable to this component).
In addition, the waste treatment of the packaging and the
product (A5, C3) plays a major role for the Climate Change -
total impact assessment indicator. In these modules, thermal
utilisation was modelled as a worst-case scenario. The large
proportion in module A5 in particular can be explained by the
fact that in addition to the waste treatment of the packaging, the
waste treatment of the protective paper is also declared in this
module, which on average accounts for one fifth of the total
mass of the product. Furthermore, both the packaging and the
protective paper contain biogenic carbon, which is accounted
for in Module A5 in the form of biogenic CO emissions.
2
7 Environmental Product Declaration - Sifloor AG - Skirting Tapes
needed to generate and provide electricity, as well as the
renewable energy resources contained in the raw materials and
packaging materials with biogenic content.
The coefficients of variation of the life cycle inventory indicators
generally show a moderate level of scatter. Among the life cycle
inventory indicators, the results for the indicators Hazardous
waste disposed, Non-hazardous waste disposed (NHWD) and
Radioactive waste disposed (RWD) show the highest scatter,
which is due to differences in the product formulations
considered.
The assumptions used to determine the reported impact
indicator results are presented in Chapter 3.3. Specific data
was used for operational activities in phases A2-A3. Raw
material inputs (A1) were mainly modelled using generic
background data sets. Raw material inputs in particular have a
major influence on all the indicators shown, so care was taken
here to use data sets that are representative in terms of
technological aspects. In order to achieve this, also data sets
In relation to the life cycle inventory indicators Total use of were used whose reference year was up to 10 years in the
renewable primary energy resources (PERT) and Total use of past, which led to an overall medium temporal
non-renewable primary energy resources (PENRT), the largest representativeness. With regard to geographical aspects, the
share of energy consumption in the life cycle occurs in the results presented in this EPD are representative for Europe.
manufacturing phase (A1-A3). Significant contributions to Activities in the downstream life cycle phases (A4-A5; C1-C3)
primary energy demand - non-renewable (PENRT) come from were modelled using scenarios, whereby assumptions were
the energy resources contained in the raw materials. The made regarding transport distance, for example. However,
largest contribution to primary energy demand - renewable these life cycle phases are not dominant for the reported impact
(PERT) is the consumption of renewable energy resources indicators.
7. Requisite evidence
Technical data sheet, Safety Data Sheet, license of EMICODE TVOC/TSVOC after 3 and 28 days.
EC1 PLUS, certificate of the German Blue Angel and other Furthermore, the emission of volatile organic compounds from
product-related information are available for download at building products in accordance with the award criteria for the
https://int.uzin.com 7.1 VOC emissions eco-label "Low-emission floor covering adhesives and other
flooring installation materials, DE-UZ 113', were determined.
TVOC* limit values EMICODE following the AgBB scheme
for EMICODE EC1 Plus (28 days [µg/m³])
Date of test report: Test report dated 04. August 2016;
Name Value Unit
TVOC (C6 - C16) ≤ 60 μg/m3 Result: The product complies with the requirements according
Sum SVOC (C16 - C22) ≤ 40 μg/m3 to the GEV test method for 'EMICODE EC 1 PLUS – very low
emissions' classification and fulfils the requirements according
R (dimensionless) ≤ 1 -
to the award basis for DE-UZ 113.
VOC without NIK ≤ 40 μg/m3
Carcinogenic Substances ≤ 1 μg/m3 AgBB scheme
The requirements on emission performance according to AgBB
TVOC* limit values BLUE ANGEL DE-UZ 113 following the for the ü-mark are automatically regarded as satisfied for
AgBB scheme (28 days [µg/m³]) products availing of EMICODE EC 1 PLUS classification.
Name Value Unit
TVOC (C6 - C16) Specific
≤ 60 μg/m3
concentration
Sum SVOC (C16 - C22) Specific
≤ 50 μg/m3
concentration
R (dimensionless) ≤ 1
VOC without LCI Specific concentration ≤ 40 μg/m3
Carcinogenic Substances Specific ≤ 1 per single
μg/m3
concentration value
Acetic acid ≤ 140 μg/m3
Formaldehyde ≤ 0.05 ppm
Other aldehydes ≤ 0.05 ppm
Test institute: WESSLING GmbH, Germany, 48341 Altenberge
Measuring process: GEV test method for determining the
emissions of volatile organic compounds from building products
according to ISO 16000-11 in a test chamber. Testing for
carcinogenic, mutagenic, reprotoxic (CMR) substances and
8 Environmental Product Declaration - Sifloor AG - Skirting Tapes
8. References
Standards:
EN 13501-1 Candidate list
DIN EN 13501-1:2019, Fire classification of construction List of substances of very high concern for Authorisation,
products and building elements - Part 1: Classification using published in accordance with Article 59(10) of the REACH
data from reaction to fire tests. Regulation, ECHA, www.echa.europa.eu/candidate-list-table
[2023]
EN 15804
EN 15804:2012+A2:2019+AC:2021, Sustainability of DGNB
construction works — Environmental Product Declarations — DGNB – German Sustainable Building Council; www.dgnb.de
Core rules for the product category of construction products. [2023]
ISO 14025 EMICODE
EN ISO 14025:2011, Environmental labels and declarations — GEV (Gemeinschaft Emissionskontrollierte Verlegewerkstoffe,
Type III environmental declarations — Principles and Klebstoffe und Bauprodukte e.V.
procedures. Düsseldorf);www.emicode.com/en [2023]
ISO 14040 EWC
DIN EN ISO 14040: 2006, Environmental management – Life European Waste Catalog established by Commission decision
cycle assessment – Principles and framework (ISO 2000/532/EC. http://www.environment-agency.gov.uk/ [2023]
14040:2006); German and English versions EN ISO
14040:2006. German AgBB
Committee for Health-related Evaluation of Building Products:
ISO 14044 health-related evaluation of emissions of volatile organic
DIN EN ISO 14044: 2006, Environmental management – Life compounds (VOC and SVOC) from building products;
cycle assessment – Requirements and guidelines (ISO www.umweltbundesamt.de/produkte/bauprodukte/agb b.htm
14044:2006); German and English versions EN ISO [2012]
14044:2006.
IBU 2021
ISO 15686 Institut Bauen und Umwelt e.V.: General Instructions for the
DIN ISO 15686:2017, Buildings and constructed assets -- EPD programme of Institut Bauen und Umwelt e.V., Version
Service life planning. DIN EN 13501. 2.0, Berlin: Institut Bauen und Umwelt e.V., www.ibu-epd.com
[2023]
ISO 16000-11
DIN EN ISO 16000-11:2006-06, Indoor air – Part 11: LCA For Experts Software
Determination of the emission of volatile organic compounds LCA For Experts Software system (Version 10) and Database
from building products and furnishings – Sampling, storage of for Life Cycle Engeneering (Content Version 2023.2). Sphera
samples and preparation of test specimens. Solutions GmbH, Leinfelden-Echterdingen [2023]
ISO 22633 LEED
DIN EN ISO 22632:2019, Adhesives - Test methods for LEED (Leadership in Energy and Environmental Design);
adhesives for floor coverings and wall coverings - https://worldgbc.org/ [2023]
Determination of dimensional changes of a linoleum floor
covering in contact with an adhesive. Ordinance on Biocide Products No. 528/2012
Regulation (EU) No 528/2012 of the European Parliament and
ISO 22635 of the Council of 22 May 2012 concerning the making available
Adhesives - Test method for adhesives for plastic or rubber on the market and use of biocidal products [2012]
floor coverings or wall coverings - Determination of dimensional
changes after accelerated ageing. PCR Part A
Product Category Rules for Building-Related Products and
Further References: Services, Part A: Calculation Rules for the Life Cycle
Assessment and Requirements on the Project report,Version
Blue Angel (DE-UZ 113) 1.3, Institut Bauen und Umwelt e.V. [08/2022]
Bundesministerium für Umwelt, Naturschutz und
Reaktorsicherheit, Umweltbundesamt, DE Deutsches Institut für PCR Part B
Gütesicherung und Kennzeichnung e.V.; Jury Ecolabel; Product Category Rules for Construction Products. Part B:
https://www.blauer-engel.de/en [2023] Dispersion adhesives and primers for floor coverings, Version
3, [06/2023]
BNB
Assessment System for Sustainable Building; https://www.bnb- REACH
nachhaltigesbauen.de/en/assessment-system/ [2023] Directive (EG) No. 1907/2006 of the European Parliament and
of the Council dated 18 December 2006 on the registration,
BREEAM evaluation, approval and restriction of chemical substances
BREEAM (Building Research Establishment Environmental (REACH), for establishing a European Agency for chemical
Assessment Methodology); substances, for amending Directive 1999/45/EC and for
https://bregroup.com/products/breeam [2023] annulment of Directive (EEC) No. 793/93 of the Council,
Directive (EC) No. 1488/94 of the Commission, Guideline
9 Environmental Product Declaration - Sifloor AG - Skirting Tapes
76/769/EEC of the Council and Guidelines 91/155/EEC, Ü-mark
93/67/EEC, 93/105/EC and 2000/21/EC of the Commission Ü-mark-Übereinstimmungszeichen; https://www.dibt.de/de
[2006] [2023]
10 Environmental Product Declaration - Sifloor AG - Skirting Tapes
Publisher
Institut Bauen und Umwelt e.V. +49 (0)30 3087748- 0
Hegelplatz 1 info@ibu-epd.com
10117 Berlin www.ibu-epd.com
Germany
Programme holder
Institut Bauen und Umwelt e.V. +49 (0)30 3087748- 0
Hegelplatz 1 info@ibu-epd.com
10117 Berlin www.ibu-epd.com
Germany
Author of the Life Cycle Assessment
Uzin Utz SE 0731 4097 0
Dieselstraße 3 nachhaltigkeit@uzin-utz.com
89079 Ulm www.uzin-utz.de
Germany
Owner of the Declaration
Uzin Utz SE 0731 4097 0
Dieselstraße 3 nachhaltigkeit@uzin-utz.com
89079 Ulm www.uzin-utz.de
Germany
11 Environmental Product Declaration - Sifloor AG - Skirting Tapes
