ENVIRONMENTAL PRODUCT DECLARATION
as per ISO 14025 and EN 15804+A2
Owner of the Declaration Sonae Arauco, S.A.
Publisher Institut Bauen und Umwelt e.V. (IBU)
Programme holder Institut Bauen und Umwelt e.V. (IBU)
Declaration number EPD-SON-20230517-IBA1-EN
Issue date 10.01.2024
Valid to 09.01.2029
Particleboard, uncoated
Sonae Arauco, S.A.
www.ibu-epd.com | https://epd-online.com
1. General Information
Sonae Arauco, S.A. Particleboard, uncoated
Programme holder Owner of the declaration
IBU – Institut Bauen und Umwelt e.V. Sonae Arauco, S.A.
Hegelplatz 1 Calle Ulises 26­18
10117 Berlin 28043 Madrid
Germany Spain
Declaration number Declared product / declared unit
EPD­SON­20230517­IBA1­EN Particleboard, uncoated, per m3
This declaration is based on the product category rules: Scope:
Wood­based panels, 01.08.2021 This document refers to particleboard manufactured in the following plants
(PCR checked and approved by the SVR) of the Sonae Arauco Group:
• Sonae Arauco Beeskow GmbH, Radinkendorfer Strasse 71,
15848 Beeskow, Germany
Issue date
• Sonae Arauco Deutschland GmbH ­ Nettgau Plant, Strohmweg
10.01.2024 1, 38489 Nettgau, Germany
• Sonae Arauco Portugal, SA, Estrada Nacional 17, nº 59 e 61,
3400­691 S.Paio de Gramaças (Oliveira do Hospital), Portugal
Valid to • Sonae Arauco South Africa (Pty) Ltd, Heidelberg Road, Rocky
Drift, White River, Republic of South Africa
09.01.2029
• Sonae Arauco España­Soluciones de Madera, S.L., Carretera
Córdoba­Valencia Km 126, Estación Linares­Baeza, 23490
Linares (Jaén), Spain
The production volume of these plants covers 100 % of the total production
of particleboard by Sonae Arauco group.
The owner of the declaration shall be liable for the underlying information
and evidence; the IBU shall not be liable with respect to manufacturer
information, life cycle assessment data and evidences.
The EPD was created according to the specifications of EN 15804+A2. In
the following, the standard will be simplified as EN 15804.
Dipl.­Ing. Hans Peters Verification
(Chairman of Institut Bauen und Umwelt e.V.)
The standard EN 15804 serves as the core PCR
Independent verification of the declaration and data according to ISO
14025:2011
internally X externally
Florian Pronold Mr Olivier Muller,
(Managing Director Institut Bauen und Umwelt e.V.) (Independent verifier)
1 Environmental Product Declaration ­ Sonae Arauco, S.A. ­ Particleboard, uncoated
2. Product
characteristics according to:
2.1 Product description/Product definition
• EN 312, Particleboards – Specifications
Particleboard is a panel­shaped wood­based material in
• EN 13986+A1, Wood-based panels for use in
accordance with EN 312, which is manufactured in a flat­
construction – Characteristics, evaluation of conformity
pressing process by means of compression under heat of small
and marking.
wood particles with adhesive. Uncoated particleboards can be
unsanded, sanded and/or profiled. Due to their various
Declaration of Performance (DoP)
densities and adhesive systems, they can display a variety of
material properties and qualities like moisture resistance, load­
For more details on technical information, please see the
bearing or others.
respective products' Declaration of Performance (DoP)
For the placing on the market in the European Union/European
available at:
Free Trade Association (EU/EFTA) (with the exception of
www.sonaearauco.com
Switzerland), Regulation (EU) 305/2011 applies. When
applicable, the products need a Declaration of Performance 2.4 Delivery status
(DOP) taking into consideration EN 13986+A1 Wood-based
Particleboard ranging in thicknesses from 6 to 46 mm can be
panels for use in construction - Characteristics, evaluation of
purchased as uncoated boards. The boards are offered in
conformity and marking and the CE­marking.
standard formats. Fixed formats are also available, and
For the application and use the respective national provisions
selected formats are offered with a tongue and groove profile.
apply.
The following table includes minimum and maximum
dimensions for the boards supplied worldwide. Some of the
2.2 Application
combinations for sizes may not be available in all markets.
The area of application for uncoated particleboard primarily
involves decorative interior furnishings and furniture
Thickness: 6 – 46 mm
manufacturing.
Width: 600 – 2800 mm
Length: 800 – 6220 mm
Particleboard can be classified into the following use classes
according to the requirements established in EN 312:
For updated information on available dimensions, please refer
P1 General purpose boards for use in dry conditions
to:
P2 Boards for interior fitments (including furniture) for use in
www.sonaearauco.com
dry conditions
P3 Non load­bearing boards for use in humid conditions 2.5 Base materials/Ancillary materials
P4 Load­bearing boards for use in dry conditions
Raw particleboard bonded with urea­formaldehyde/melamine­
P5 Load­bearing boards for use in humid conditions
urea­formaldehyde (UF/MUF) consist of (dimensions as % by
P6 Heavy duty load­bearing boards for use in dry conditions
mass):
P7 Heavy duty load­bearing boards for use in humid conditions
• Wood chips: approx. 85 %
2.3 Technical Data • Water: 4 – 7 %
Due to the large variability of product properties and quality • UF glue / MUF glue (urea resin, melamine urea resin): 8
grades, the table below only shows the range of technical – 10 %
characteristics for classes P1 to P3 (boards for non­structural • Paraffin wax emulsion: < 1.5 %
applications). Raw particleboard bonded with polymeric diphenylmethane
diiscocyanate (PMDI) consist of (dimensions as % by mass):
Structural boards as well as customized products have different • Wood chips: approx. 85 %
technical characteristics from the ones shown. • Water: 4 – 7 %
Name Value Unit • PMDI (polymer 4.4' diphenyl methane diisocyanate)
Bending strength (longitudinal) according to glue: 4 – 6 %
EN 310 5.5 ­ 15 N/mm2 • Paraffin wax emulsion: < 1.5%
Wood from indigenous, largely regional forest plantations is
1050 ­
E­module (longitudinal) according to EN 310 N/mm2 used for manufacturing raw particleboard. This wood is typically
1950
procured from forests within an average radius of 250 km of the
Tensile strength rectangular according to EN 0.14 ­
N/mm2 plants' locations.
319 0.45
Density limit deviation from average value Furthermore, sawmill residues and recycled wood are also
+/­ 10 %
according to EN 323 used as key raw materials in the production of particleboard.
Thickness tolerance (sanded) according to
+/­ 0.3 mm
EN 324 The entire particleboard range can be made available on
Length and with tolerance according to EN request as FSC® certified or PEFC (program for the
+/­ 5.0 mm
324 endorsement of forest certification) certified products.
Edge straightness tolerance according to EN
324 +/­ 1.5 mm/m This product contains substances listed in the ECHA candidate
list (date: 08.06.2021) exceeding 0.1 percentage by mass: no
Perpendicularity according to EN 324 +/­ 2.0 mm/m
Thickness swelling according to EN 317 12 ­ 17 %
This product contains other carcinogenic, mutagenic or
Moisture content according to EN 322 5 ­ 13 % reprotoxic (CMR) substances in categories 1A or 1B which are
not on the ECHA candidate list, exceeding 0.1 percentage by
Performance data of the product in accordance with the
mass: no
declaration of performance with respect to its essential
2 Environmental Product Declaration ­ Sonae Arauco, S.A. ­ Particleboard, uncoated
Biocide products were added to this construction product or it pressure in a hot press. The panels are trimmed, picked and
has been treated with biocide products (this then concerns a sanded on both sides after cooling.
treated product as defined by the (EU) Regulation on biocidal
products No. 528/2012: no All leftovers incurred during board manufacture are redirected
into the process or used as fuel to supply the energy needs of
2.6 Manufacture the manufacturing process on site.
The wood is chipped, screened and dried. Surface layer and
core layer materials are then glued and scattered on a forming A process diagram is presented below.
belt as a particles' mat. This is pressed into panels under high
The production sites are all ISO 14001 certified.
2.8 Product processing/Installation
The production sites are certified according to the following Sonae Arauco particleboard can be sawn, milled, planed,
standards: sanded and drilled using standard machinery or (electric) power
tools. Carbide­tipped tools should be given preference,
• ISO 9001
especially on circular saws. Respiratory protection should be
• ISO 45001
worn when using hand­held equipment without suction devices.
• EN ISO 50001 (European sites).
Please refer to the respective devices' datasheets for further
2.7 Environment and health during manufacturing processing recommendations.
Health protection: Due to the manufacturing conditions, no
2.9 Packaging
special health protection measures over and beyond the
Sonae Arauco particleboards are supplied on squared timber
regulatory guidelines are required. The reference occupational
bound by plastic or metal bands and covered with corrugated
exposure limit values are complied with.
cardboard and, on the bottom, with a cover board.
Particleboard and steel or PET packing bands for transport
Emissions into air: Waste air generated during production is
packaging can be sorted and directed to the recycling circuits. If
cleaned in accordance with regulatory requirements. Emissions
re­use or recycling is impractical, the packaging should not be
have to comply with the values specified by the operation
landfilled, but rather directed towards energy recovery.
licenses of the different sites, specified according to national
Packaging disposal information is available at:
laws.
www.sonaearauco.com
Emissions into water/soil: No normal process contamination 2.10 Condition of use
of water or soil exists. Typically, the production process of
The components making up uncoated particleboard correspond
particleboard does not have any production­related waste
with the base material compositions
water.
as outlined in section 2.6. During hot pressing, the binding
agent is linked irreversibly by means of poly­condensation and
Noise: Noise surveys are required and are performed for each
firmly bonded with the wood. The binding agents are chemically
site according to respective national regulations. Noise­
and stably bound to the wood.
intensive plant areas such as chipping are encapsulated or
protected appropriately by structural measures. Whenever
VOC emissions: Sonae Arauco particleboards are labelled as
necessary (close to non­encapsulated areas), the use of ear
class A or B according to the French regulation on the labelling
protection is required (PPE, Personal Protective Equipment)
of emissions of volatile pollutants from construction and
within Sonae Arauco sites, as an additional safety measure.
decoration products (with reference to the wall scenario, as a
worst case).
3 Environmental Product Declaration ­ Sonae Arauco, S.A. ­ Particleboard, uncoated
Sonae Arauco particleboard at an average density of 659,4 Water
kg/m3 stores 1000 kg CO equivalent over its service life. No ingredients are washed out which could be hazardous to
2
water. Particleboards are not resistant to permanent exposure
2.11 Environment and health during use to water.
Environmental protection: According to current information,
water, air and soil are not exposed to any dangers when the Mechanical destruction
respective products outlined above are used as designated. Mechanical destruction of particleboards can result in sharp
edges on the broken panel edges (risk of injury).
Health protection: According to current information, no
2.14 Re-use phase
damage to or impairment of health can be anticipated when
Recycling: Sonae Arauco particleboards from construction can
particleboards are used as designated.
be collected separately and utilised in the manufacture of
particleboard. This is based on the condition that the wooden
With the exception of low volumes of formaldehyde for
boards are not
UF/MUF­bonded particleboard, VOC emissions from products
fully glued.
are negligible, and are natural wood ingredients.
Energy recovery: Due to the high heating value of approx.
2.12 Reference service life 16.0 MJ/kg at 20 % moisture content assumed for post­
Due to the wide range of applications of Sonae Arauco consumer boards, particleboards can be used for energy
particleboard, no reference service life is declared. recovery and the generation of heat and electricity (e.g., in CHP
plants), following the cascading principle for wood.
2.13 Extraordinary effects
2.15 Disposal
Fire
Fire retardant classification of particleboard is done according Sonae Arauco particleboard leftovers and residual materials
to EN 13986. Fire retardant classes are defined in accordance incurred as a result of demolition measures on the building sites
with EN 13501-1. should be primarily directed towards material recycling. If this is
not possible, they must be directed toward energy recovery
Fire protection
instead of landfilling.
Name Value
Building material class D Waste code according to the Regulation on the European
Smoke gas development S2 Waste List: 17 02 01
Burning droplets d0
2.16 Further information
Particleboards with improved fire resistance is available with Further information such as technical datasheets, etc. can be
classification B­s2,d0 downloaded under:
www.sonaearauco.com
3. LCA: Calculation rules
Module A4 covers the transport of the product from the
3.1 Declared Unit production site to the construction site by a lorry over a default
The declared unit for the LCA is 1 m3 of uncoated average distance of 460 km.
Sonae Arauco particleboard.
Module A5 covers the transport of the packaging material from
Information on the declared unit
the construction site and its disposal. Default end­of­waste
Name Value Unit
states for the packaging materials from the packed products at
Declared unit 1 m3 the construction site are defined in analogy for wastes
Mass reference 659.4 kg/m3 occurring in modules A1 – A3. Eventual further inputs for the
installation of the products are not considered due to the broad
The weighted average was calculated based on production
applicability of the assessed products.
volumes from the plants in all countries where Sonae Arauco
The substituted primary material from the net amount of
was operating in 2021 (some plants 2020).
recycled material and from recovered energy exported from the
product system in Module A5 is declared in Module D.
3.2 System boundary
Type of the EPD: cradle­to­gate with modules C1 to C4 and
Module C1 manual deconstruction is assumed. The declared
module D (A1 – A3, C and D)
values are thus 0.
Modules A1 – A3 of the production stage cover the
Module C2 includes the transport of the de­constructed product
manufacturing of the products, including raw material extraction
to a recycling centre by over 50 km.
and processing, energy generation, the production of ancillary
products and packaging materials, transport, as well as all
Module C3 covers the preparation of the post­consumer board
waste treatment processes. Eventual benefits of recycling or
to become a secondary fuel; the end­of­waste status for
energy recovery are neglected.
recycled wood­based boards is defined as the point where they
The resource aspects of wood were inventoried via material
have been sorted and chipped, ready to be used as secondary
inherent properties such as resource extraction of CO from the
2 fuels.
atmosphere and the lower heating value as the use of
In line with EN 16485, the export of the biogenic carbon stored
renewable energy. Material inherent properties are subject to
in the board, expressed in CO ­equivalent is also reported in
2
co­product allocation as ruled in EN 15804.
module C3.
4 Environmental Product Declaration ­ Sonae Arauco, S.A. ­ Particleboard, uncoated
Module C4 is not relevant for the assumed end­of­life scenario. • Datasets are based on 1­year averaged data as a
The declared values are thus 0. general rule;
• The time period over which inputs to and outputs from
Module D compiles all the benefits and burdens associated with the system are accounted for is 100 years from the year
the secondary fuels, secondary materials and exported energy for which the data set is deemed representative;
leaving the production system in the modules A5 and C3. • The technological coverage reflects the physical reality
Therefore, module D covers the avoided burdens from recycling of the declared products;
and from energy recovered from the waste treatment in module • The background datasets comply with the quality
A5 as well as the transport of the obsolete boards to a biomass guidelines of ecoinvent v.3; deviations from the
combustion plant, the combustion process itself and the loads methodological prescriptions of EN 15804 cannot be
and benefits of the substitution of fossil fuels and/or electricity. excluded but are considered not significant in the
Substitution effects in module D are always calculated for the context of this EPD.
net amount of secondary material or secondary fuel of the
product system in line with EN 16485. 3.7 Period under review
The company data gathered for this EPD represents the year
3.3 Estimates and assumptions 2020/21.
For the quantification of the net flows of recycled wood (input of
post­consumer wood used as a fuel minus post­consumer 3.8 Geographic Representativeness
wood exiting the product system into module D for energy Land or region, in which the declared product system is
recovery), it was assumed that all inputs of post­consumer manufactured, used or handled at the end of the product´s
wood are used as a fuel; inputs of post­consumer wood beyond lifespan: Europe
the need of wood fuel used in production was considered to be
used as a recycled material input. Beyond that, no relevant
3.9 Allocation
estimates or assumptions had to be made further to the
The inventories for the wood inputs were taken from ecoinvent
information provided in this EPD.
v.8. In ecoinvent, the forestry processes are modelled on a
3.4 Cut-off criteria mass­basis and sawmilling processes are allocated based on
All data were taken into account that resulted from the data revenues of the different co­products of a joint co­production
collection procedure in the plants, e.g. related to fuels, raw process.
material input, use of ancillary materials, waste flows, Waste generated by edge­trimming and cut­size saws is used
emissions into the air, water use, waste water, transport means internally for energy generation. Some plants sell minor
and transport distances, etc.. quantities of bark, waste wood or electricity from co­generation.
Expenses for the general management, research & No impacts are allocated to these outputs.
development, administration and marketing – if known – were Biogenic carbon (content) is modelled manually thus reflects
not taken into account. the real physical flows; this is not the case for primary energy,
The production of eventual packaging of ancillary material or implying that the content of primary energy in products and
other inputs used during production (and some of the reported packaging is allocated as the main inputs/outputs of a unit
wastes) were generally neglected; in most cases reusable bins process.
or containers are used. In addition, the amounts of reported In the case of sites where several products were produced and
(unspecific) wastes are so small that their production can be no product­specific information was available, all inputs and
considered not relevant for the life cycle assessment. Additional outputs related to production processes were attributed based
plant specific information can be found in the respective on a total mass of production; packaging material was
chapters for each plant. attributed based on a total volume of the production. Inputs and
Beyond that some plants reported ancillary materials that were outputs for coating processes that could not be separated from
cut off due to very small amounts and as inputs not directly the data on plant level were conservatively attributed to the
related to production processes but to the maintenance of particleboard production.
infrastructure, e.g. acetylene and oxygen for soldering, etc. Post­consumer secondary wood is used as an input to produce
With this approachmass and energy flows below 1 percent of particleboard; for this input as well as for the end­of­life
total mass and energy flows caused by the declared products scenario, the end­of­waste status was defined after the sorting
were included in the assessment. and chipping of the wood­based board in line with EN 16485
Beyond that, no material or energy flows were neglected that (see also clause 3.2). In analogy, particleboard leaving the
would have been known by the persons responsible for the product system at the end­of­life is considered a secondary
project and that could have been expected to contribute fuel; its combustion and the benefits of energy recovery are
significantly to the environmental indicators declared. It can declared in module D.
thus be assumed that the total contribution of the neglected Waste packaging in module A5 was considered not to reach the
processes is not higher than 5 % of the declared impact end­of­waste state as a fuel. Its incineration is reported in A5,
categories. the benefits of energy recovery in module D. The benefits of the
recycling of minor amounts of packaging materials are
3.5 Background data disregarded.
Datasets from ecoinvent v3.8 were used as background data No co­product allocation was made in the modelling of the
exclusively. Therefore, the latest update of the background data foreground data of the life cycle assessment underlying this
took place in 2021. EPD.
3.6 Data quality 3.10 Comparability
The requirements on the data quality and the background data Basically, a comparison or an evaluation of EPD data is only
correspond to the provisions in EN 15804: possible if all the data sets to be compared were created
according to EN 15804 and the building context, respectively
• Data are as current as possible. Datasets used for
the product­specific characteristics of performance, are taken
calculations were updated within the last 10 years for
into account. Datasets from ecoinvent v3.8 were used as
generic data and within the last 5 years for producer­
background data exclusively.
specific data;
5 Environmental Product Declaration ­ Sonae Arauco, S.A. ­ Particleboard, uncoated
4. LCA: Scenarios and additional technical information
Deconstruction (C1)
Characteristic product properties of biogenic carbon Manual deconstruction is assumed. The declared values are
Note: 1 kg of biogenic carbon is equivalent to 44/12 kg of CO 2. thus 0.
Information on describing the biogenic carbon content at
Transport to waste treatment (C2)
factory gate
This module includes the transport of the de­constructed
Name Value Unit
product to a recycling centre by a lorry (15 % emissions class
Biogenic carbon content in product 272.9 kg C EURO 5; 85 % emissions class EURO 6) by over 50 km.
Biogenic carbon in packaging 3.43 kg C
Waste treatment (C3)
731 kg of particleboard a chipped and exported from the
Transport to the construction site (A4)
product life cycle into module D, assuming a moisture content
The product is transported from the production site to the
of 20 % and a lower heating value of 16.2 MJ/kg. The biogenic
construction site by a lorry (15 % emissions class EURO 5; 85
carbon stored in the product and the content of primary energy
% emissions class EURO 6) over a default distance of 460 km.
are exported from the product system as material inherent
properties.
Installation into the building (A5)
Eventual further inputs for the installation of the products are
Disposal (C4)
not considered due to the broad applicability of the assessed
This module is not relevant for the assumed end­of­life
products.
scenario. The declared values are thus 0.
An average transport distance of 30 km was assumed for
packaging waste from the construction site to the recycling
Reuse, recycling, recovery potential (D)
plant or to the municipal waste incineration plant. The municipal
According to default assumptions in other IBU EPDs, post­
waste incineration plant is assumed to have an overall energy
consumer wood is used as a secondary fuel for energy
efficiency of 53 % related to the lower heating value of the
recovery in a biomass combustion plant with an overall energy
waste input; 92 % of the recovered energy is heat, 8 % is
efficiency of 93 % related to the lower heating value of the fuel
electricity (according to specifications of MWI plants in
input; 91 % of the recovered energy is heat, 9 % is electricity.
ecoinvent v3.8).
6 Environmental Product Declaration ­ Sonae Arauco, S.A. ­ Particleboard, uncoated
5. LCA: Results
DESCRIPTION OF THE SYSTEM BOUNDARY (X = INCLUDED IN LCA; MND = MODULE OR INDICATOR NOT DECLARED; MNR
= MODULE NOT RELEVANT)
Benefits and
Construction loads beyond
Product stage Use stage End of life stage
process stage the system
boundaries
la ire ta m w a Ry lp p u s tro p s n a rT g n iru tc a fu n a M e h t m o rf tro p s n a rTe tis e h t o t e ta g y lb m e s s A e s U e c n a n e tn ia M ria p e R tn e m e c a lp e R tn e m h s ib ru fe R y g re n e la n o ita re p Oe s u re ta w la n o ita re p Oe s u n o itc u rts n o c ­e Dn o itilo m e d tro p s n a rT g n is s e c o rp e ts a W la s o p s iD ­e s u e R­y re v o c e R­g n ilc y c e Rla itn e to p
A1 A2 A3 A4 A5 B1 B2 B3 B4 B5 B6 B7 C1 C2 C3 C4 D
X X X X X MND MND MNR MNR MNR MND MND X X X X X
RESULTS OF THE LCA - ENVIRONMENTAL IMPACT according to EN 15804+A2: Particleboard, uncoated, per m³
Parameter Unit A1-A3 A4 A5 C1 C2 C3 C4 D
GWP­total kg CO 2 eq ­6.82E+02 5.03E+01 1.36E+01 0 7.04E+00 1.01E+03 0 ­3.21E+02
GWP­fossil kg CO 2 eq 3.31E+02 5.02E+01 1.03E+00 0 7.04E+00 5.94E+00 0 ­3.2E+02
GWP­biogenic kg CO 2 eq ­1.01E+03 0 1.26E+01 0 0 1E+03 0 0
GWP­luluc kg CO 2 eq 5.49E­01 2E­02 1.07E­04 0 3.33E­03 1.36E­02 0 ­1.83E­01
ODP kg CFC11 eq 4.95E­05 1.16E­05 9.99E­08 0 1.59E­06 2.98E­07 0 ­6.73E­05
AP mol H+ eq 2.09E+00 1.52E­01 4.87E­03 0 2.11E­02 3.17E­02 0 ­5.25E­01
EP­freshwater kg P eq 1.27E­02 3.57E­04 3.44E­06 0 5.74E­05 6.16E­04 0 ­8.1E­03
EP­marine kg N eq 3.68E­01 3.33E­02 2.15E­03 0 4.43E­03 4.31E­03 0 ­5.59E­02
EP­terrestrial mol N eq 4.91E+00 3.7E­01 2.42E­02 0 4.94E­02 4.92E­02 0 ­6.23E­01
kg NMVOC
POCP 1.4E+00 1.34E­01 7.2E­03 0 1.79E­02 1.39E­02 0 ­2.72E­01
eq
ADPE kg Sb eq 4.06E­03 1.78E­04 9.68E­07 0 3.22E­05 1.63E­05 0 ­1.97E­04
ADPF MJ 6.64E+03 7.61E+02 5.69E+00 0 1.05E+02 1.24E+02 0 ­8.8E+03
m3 world eq
WDP 3.74E+02 2.31E+00 5.55E­02 0 3.49E­01 1.44E+00 0 ­9.59E+00
deprived
GWP = Global warming potential; ODP = Depletion potential of the stratospheric ozone layer; AP = Acidification potential of land and water; EP =
Eutrophication potential; POCP = Formation potential of tropospheric ozone photochemical oxidants; ADPE = Abiotic depletion potential for non­fossil
resources; ADPF = Abiotic depletion potential for fossil resources; WDP = Water (user) deprivation potential)
RESULTS OF THE LCA - INDICATORS TO DESCRIBE RESOURCE USE according to EN 15804+A2: Particleboard, uncoated,
per m³
Parameter Unit A1-A3 A4 A5 C1 C2 C3 C4 D
PERE MJ ­6.47E+03 1.07E+01 1.68E+02 0 1.75E+00 2.15E+01 0 ­2.9E+02
PERM MJ 1.05E+04 0 ­1.68E+02 0 0 ­1.04E+04 0 0
PERT MJ 4.07E+03 1.07E+01 1.02E­01 0 1.75E+00 ­1.04E+04 0 ­2.9E+02
PENRE MJ 4.99E+03 7.62E+02 1.38E+01 0 1.05E+02 1.25E+02 0 ­8.72E+03
PENRM MJ 1.66E+03 0 ­8.09E+00 0 0 ­1.65E+03 0 0
PENRT MJ 6.65E+03 7.62E+02 5.69E+00 0 1.05E+02 ­1.53E+03 0 ­8.72E+03
SM kg 1.63E+02 0 0 0 0 0 0 0
RSF MJ 4.19E+03 0 0 0 0 0 0 6.19E+03
NRSF MJ 0 0 0 0 0 0 0 1.65E+03
FW m3 9.79E+00 8.06E­02 5.05E­03 0 5.05E­03 7.56E­02 0 ­6.96E­01
PERE = Use of renewable primary energy excluding renewable primary energy resources used as raw materials; PERM = Use of renewable primary
energy resources used as raw materials; PERT = Total use of renewable primary energy resources; PENRE = Use of non­renewable primary energy
excluding non­renewable primary energy resources used as raw materials; PENRM = Use of non­renewable primary energy resources used as raw
materials; PENRT = Total use of non­renewable primary energy resources; SM = Use of secondary material; RSF = Use of renewable secondary fuels;
NRSF = Use of non­renewable secondary fuels; FW = Use of net fresh water
RESULTS OF THE LCA – WASTE CATEGORIES AND OUTPUT FLOWS according to EN 15804+A2:
Particleboard, uncoated, per m³
Parameter Unit A1-A3 A4 A5 C1 C2 C3 C4 D
HWD kg 8.95E­03 1.99E­03 4.72E­06 0 2.82E­04 5.76E­05 0 ­9.51E­03
NHWD kg 6.98E+01 4E+01 1.37E­01 0 4.51E+00 8.2E­01 0 7.74E+00
RWD kg 2.93E­02 1.1E­02 7.49E­05 0 1.51E­03 1.62E­03 0 ­2.78E­02
CRU kg 0 0 0 0 0 0 0 0
MFR kg 7.84E­01 0 7.1E­01 0 0 0 0 0
MER kg 0 0 0 0 0 7.32E+02 0 0
EEE MJ 2.72E­02 0 5.82E+00 0 0 0 0 0
EET MJ 3.12E­01 0 6.69E+01 0 0 0 0 0
7 Environmental Product Declaration ­ Sonae Arauco, S.A. ­ Particleboard, uncoated
HWD = Hazardous waste disposed; NHWD = Non­hazardous waste disposed; RWD = Radioactive waste disposed; CRU = Components for re­use;
MFR = Materials for recycling; MER = Materials for energy recovery; EEE = Exported electrical energy; EET = Exported thermal energy
RESULTS OF THE LCA – additional impact categories according to EN 15804+A2-optional:
Particleboard, uncoated, per m³
Parameter Unit A1-A3 A4 A5 C1 C2 C3 C4 D
Disease
PM 1.49E­05 3.22E­06 6.8E­08 0 3.87E­07 9.66E­08 0 ­5.6E­07
incidence
IR kBq U235 eq 1.32E+01 3.31E+00 2.28E­02 0 4.58E­01 1.09E+00 0 ­1.6E+01
ETP­fw CTUe 7.89E+03 5.97E+02 1.14E+01 0 8.6E+01 7.03E+01 0 ­6.41E+02
HTP­c CTUh 2.48E­06 1.92E­08 2.55E­09 0 3.11E­09 3.33E­09 0 7.58E­08
HTP­nc CTUh 6.19E­06 6.07E­07 1.11E­08 0 8.38E­08 6.04E­08 0 6.18E­09
SQP SQP 2.06E+04 5.3E+02 1.16E+00 0 6.23E+01 1.91E+01 0 ­2.6E+02
PM = Potential incidence of disease due to PM emissions; IR = Potential Human exposure efficiency relative to U235; ETP­fw = Potential comparative
Toxic Unit for ecosystems; HTP­c = Potential comparative Toxic Unit for humans (cancerogenic); HTP­nc = Potential comparative Toxic Unit for humans
(not cancerogenic); SQP = Potential soil quality index
Disclaimer 1 – for the indicator “Potential Human exposure efficiency relative to U235”. This impact category deals mainly with the
eventual impact of low­dose ionizing radiation on human health of the nuclear fuel cycle. It does not consider effects due to possible
nuclear accidents, occupational exposure or radioactive waste disposal in underground facilities. Potential ionizing radiation from the
soil, radon and from some construction materials is also not measured by this indicator.
Disclaimer 2 – for the indicators “abiotic depletion potential for non­fossil resources”, “abiotic depletion potential for fossil resources”,
“water (user) deprivation potential, deprivation­weighted water consumption”, “potential comparative toxic unit for ecosystems”,
“potential comparative toxic unit for humans – cancerogenic”, “Potential comparative toxic unit for humans ­ not cancerogenic”,
“potential soil quality index”. The results of this environmental impact indicator shall be used with care as the uncertainties on these
results are high as there is limited experience with the indicator.
6. LCA: Interpretation
Figure 1 illustrates the contribution of each life cycle stage to from module A1 – C4 = 100 %) for uncoated particleboard.
the overall indicator results of the impact assessment (impact
construction site whereas the contributions from other modules
Figure 1: Environmental impacts of uncoated particleboard of the life cycle are negligible.
along its life cycle (impacts from production modules A1 – Loads and benefits beyond the life cycle (module D) are
C4 = 100 %) negative (benefits > loads) whereas major contributions occur
for the ODP, the GWP­fossil and for the ADPF; these benefits
Figure 1 illustrates that the environmental profile of uncoated basically stem from the use of the particleboard as secondary
particleboard is dominated by the production phase (modules fuel and its related substitution of natural gas and electricity
A1 – A3). Minor contributions stem from transport to the from the grid from the recovered energy.
8 Environmental Product Declaration ­ Sonae Arauco, S.A. ­ Particleboard, uncoated
Figure 2 illustrates that the biogenic carbon stored in the
uncoated particleboard, expressed as CO ­equivalent, is higher
2
than the CO emissions from fossil sources, leading to a
2
negative GWP for the production module A1 – A3. The potential
substitution effect in mod­ule D almost offsets the greenhouse
gas emissions during the production phase (module A1 – A3).
Figure 2: Greenhouse Gas balance of uncoated
particleboard
The GWP is dominated by CO emissions and removals.
2
7. Requisite evidence
7.1 Formaldehyde Cologne, Germany
Test reports, date: Report 0001122970/20 AZ 581067,
For UF/MUF bonded boards: 20.09.2022
(tests made on raw boards) Result: The limit values are complied with. Limits evaluated
Measuring agency: MPA Eberswalde materialprüfanstalt according to the Toy safety-directive 2009/48/EC: category 3:
Brandenbutg GmbH ­ Holz uns Holzschutz Scraped of toy material.
Test report, date: No 31/23/4155/01/QT issued at 02.04.2023
Result: ZE05 ­ Certification of wood­based panels regarding Metal analysis for Iberian market, based on quarterly analysis:
formaldehyde emissions in accordance with the German Measuring agency: IDIT, Instituto de Desenvolvimento e
Chemicals Prohibition Ordinance (ChemVerbotsV) and based Inovação Tecnológica, Portugal
on DIBt Guideline 100. Test procedure according to DIN EN Test reports, date: 2057/2015 & 2058/2015, 22 December
717-1. 2015
Calculated formaldehyde concentration was 0,054 ppm Result: The limit values outlined in the EPF voluntary
according to ChemVerbotsV (concentration of EN 717-1 standards on the use of recycled wood are complied with. Limit
multiplied by factor 2), compying with the limit 0,1ppm. values in mg/kg: As 25, Pb 90, Cd 50, Cr 25, Cu 40, Hg 25, Cl
1000, F 100, PCP 5 and Creosote 0.5. .
Measuring agency: MPA Eberswalde materialprüfanstalt
Brandenbutg GmbH ­ Holz uns Holzschutz 7.3 TVOC emissions
Test report, date: No. 31/23/3768/01/QT issued on the
25.01.2023 (tests made on raw boards)
Result: ZE05 ­ Certification of wood­based panels regarding Measuring agency: MPA Eberswalde materialprüfanstalt
formaldehyde emissions in accordance with the German Brandenbutg GmbH ­ Holz uns Holzschutz
Chemicals Prohibition Ordinance (ChemVerbotsV) and based Test report, date: Nr 31/22/4843/01 dated 01.09.2022
on DIBt Guideline 100. Test procedure according to DIN EN Result:
717-1. Emissions tested for PB P4. Requirements for AgBB achived
Calculated formaldehyde concentration was 0,045 ppm for both 3 and 28 days.
according to ChemVerbotsV (concentration of EN 717­1
multiplied by factor 2), compying with the limit 0,1ppm AgBB overview of results (28 days [µg/m³])
Name Value Unit
Measuring agency: Fraunhofer Institute for Wood Research
TVOC (C6 ­ C16) 550.0 μg/m3
Wilhelm­Klauditz­Institut WKI
Test report, date: No. QA­2021­0453 issued on the 04.03.2021 Sum SVOC (C16 ­ C22) < 5 μg/m3
Results: Determination of the formaldehyde release according R (dimensionless) 1 ­
to JIS A1460. An average value of 0,1 mg/litre was determined VOC without NIK 97 μg/m3
with individual values of 0,06 mg/litre and 0,09 mg/litre
Carcinogenic Substances < 1 μg/m3
corresponding to the F4Stars level
Formaldehyde 48 µg/m3
7.2 Checking for the pretreatment of the substances used
The VOC measurements allowed for a classification A+, when
excluding formaldehyde (class A, when taking formaldehyde
(tests made on raw boards)
emissions into consideration).
Measuring agency: TÜV Rheinland LGA Products GmbH,
9 Environmental Product Declaration ­ Sonae Arauco, S.A. ­ Particleboard, uncoated
Measuring agency: EPH Entwicklungs­ und Prüflabor
AgBB overview of results (3 days [µg/m³])
Holztechnologie GmbH, Zellescher Weg 24, D­01217 Dresden
Name Value Unit
Test reports, date: Report no. 2522491/1/A2 dated 15­12­
TVOC (C6 ­ C16) ­ μg/m3 2022
Carcinogenic Substances < 1 μg/m3 Result: Value of 0.6 mg/kg was determined for PCP.
Lindane was not detected.
The requirements considered for PCP (mg/kg) and Lindane
7.4 PCP/Lindane
(mg/kg) were all fulfilled, with determined values below the max
values.
(tests made on raw boards)
8. References
Product category rules of IBU EN 12524
EN 12524:2000, Building materials and products –
IBU (2021) Hygrothermal properties – Tabulated design values.
IBU (2021): General Instructions for the EPD Programme of the
Institut Bauen und Umwelt e.V. (General Instructions for the EN 13501
IBU EPD Programme). Version 2.0, Institut Bauen und Umwelt EN 13501­1:2019, Fire classification of construction products
e.V., Berlin. and building elements – Classification using test data from
reaction to fire tests.
IBU (2021)
IBU (2021): PCR Part A: Calculation rules for the life cycle EN 13986
assessment and requirements for the project report according EN 13986:2015, Wood­based panels for use in construction –
to EN 15804+A2:2019. Version 1.3, Institut Bauen und Umwelt Characteristics, evaluation of conformity and marking.
e.V., Berlin. EN 15804
EN 15804+A2:2019+ AC:2021, Sustainability of construction
IBU (2023) works – Environmental product declarations – Core rules for the
IBU (2023): PCR Part B: Requirements on the EPD for wood­ product category construction products.
based panels. Version 2023/04, Institut Bauen und Umwelt e.V.,
Berlin. EN 16485
EN 16485:14­07, Round and sawn timber – Environmental
Standards and legal documents Product Declarations – Product category rules for wood and
wood­based products for use in construction.
EN 310
EN 310:1993, Wood­based panels – Determination of modulus ISO 9001
of elasticity in bending and of bending strength. ISO 9001:2015, Quality management systems – Requirements.
EN 312 ISO 14025
EN 312:2010, Particleboards – Specifications. ISO 14025:2006­07, Environmental labels and declarations –
Type III Environmental declarations – Principles and
EN 317 procedures.
EN 317:1993, Particleboards and Fibreboards – Determination
of swelling in thickness after immersion in water. ISO 14044
EN ISO 14044:2006­07, Environmental management – Life
EN 319 cycle assessment – Requirements and guidance.
EN 319:1993, Particleboards and fibreboards – Determination
of tensile strength perpendicular to the plane of the board. ISO 14001
ISO 14001:2015, Environmental management systems –
EN 322 Requirements with guidance for use.
EN 322:1993, Wood­based panels – Determination of moisture
content. ISO 14025
ISO 14025:2006­07, Environmental labels and declarations –
EN 323 Type III Environmental declarations – Principles and
EN 323:1993, Wood­based panels – Determination of density. procedures.
EN 324 ISO 14044
EN 324­1:1993, Wood­based panels – Determination of EN ISO 14044:2006­07, Environmental management – Life
dimensions of boards – Determination of thickness, width and cycle assessment – Requirements and guidance.
length.
EN 324­2:1993, Wood­based panels – Determination of ISO 16000
dimensions of boards – Determination of squareness and edge ISO 16000­11:2006, Indoor air – Part 11: Determination of the
straightness. emission of volatile organic compounds from building products
and furnishing – Sampling, storage of samples and preparation
EN 717-1 of test specimens.
EN 717­1:2005­01, Wood­based panels – Determination of
formaldehyde release – Formaldehyde emission by the ISO 45001
chamber method. DIN ISO 45001:2018­06, Occupational health and safety
management systems – Requirements with guidance for use.
10 Environmental Product Declaration ­ Sonae Arauco, S.A. ­ Particleboard, uncoated
ISO 50001 Regulation on biocidal products
ISO 50001:2018, Energy management systems – REGULATION (EU) No 528/2012 OF THE EUROPEAN
Requirements with guidance for use. PARLIAMENT AND OF THE COUNCIL of 22 May 2012
concerning the making available on the market and use of
JIS A 1460 biocidal products.
JIS A 1460:2015: Determination of the emissions of
formaldehyde from building boards – Desiccator method. Regulation (EU) Nr. 305/2011(CPR)
REGULATION (EU) No 305/2011 OF THE EUROPEAN
ChemVerbotsV PARLIAMENT AND OF THE COUNCIL of 9 March 2011 laying
Verordnung über Verbote und Beschränkungen des down harmonised conditions for the marketing of construction
Inverkehrbringens und über die Abgabe bestimmter Stoffe, products and repealing Council Directive 89/106/EEC.
Gemische und Erzeugnisse nach dem Chemikaliengesetz
(Chemikalien­Verbotsverordnung ­ ChemVerbotsV); Regulation on the European Waste List (Waste index)
Ausfertigungsdatum: 20.01.2017. http://www.gesetze­im­internet.de/avv/anlage.html
COUNCIL REGULATION (EU) No 333/2011 Toy safety-directive 2009/48/EC
COUNCIL REGULATION (EU) No 333/2011 of 31 March 2011 Directive 2009/48/EC of the European Parliament and of the
establishing criteria determining when certain types of scrap Council of 18 June 2009 on the safety of toys (Text with EEA
metal cease to be waste under Directive 2008/98/EC of the relevance).
European Parliament and of the Council.
Additional references
DIBt Guideline 100
Regulation on the classification and external supervision of BBSR 2017
wood­based panels regarding formaldehyde emission (DIBt ­ Bundesinstitut für Bau­, Stadt­ und Raumforschung Service Life
Guideline 100), dated June 1994. of Building Components; version 24.02.2017.
ECHA candidate list https://www.nachhaltigesbauen.de/fileadmin/pdf/Nutzungsdauer_Bauteile/BNB_Nutzungsdauern_von_Bauteilen_2017­
The Candidate List of substances of very high concern 2­24.pdf
published by the European Chemicals Agency (ECHA),
Helsinki, available via https://echa.europa.eu/nl/­/four­ ecoinvent v3.8
newsubstances­added­to­the­candidate­list. LCA database ecoinvent v3.8, 12/2021. ecoinvent centre,
Zürich.
11 Environmental Product Declaration ­ Sonae Arauco, S.A. ­ Particleboard, uncoated
Publisher
Institut Bauen und Umwelt e.V. +49 (0)30 3087748­ 0
Hegelplatz 1 info@ibu­epd.com
10117 Berlin www.ibu­epd.com
Germany
Programme holder
Institut Bauen und Umwelt e.V. +49 (0)30 3087748­ 0
Hegelplatz 1 info@ibu­epd.com
10117 Berlin www.ibu­epd.com
Germany
Author of the Life Cycle Assessment
Dr. Frank Werner ­ Umwelt & Entwicklung + 41 (0)44 241 39 06
Kammelenbergstrasse 30 frank@frankwerner.ch
9011 St. Gallen http://www.frankwerner.ch/
Switzerland
Owner of the Declaration
Sonae Arauco, S.A. (+34) 918 070 701
Calle Ulises 26­18 products@sonaearauco.com
28043 Madrid www.sonaearauco.com
Spain
12 Environmental Product Declaration ­ Sonae Arauco, S.A. ­ Particleboard, uncoated
