ENVIRONMENTAL PRODUCT DECLARATION
as per ISO 14025 and EN 15804+A2
Owner of the Declaration Kima Accessories Aps
Publisher Institut Bauen und Umwelt e.V. (IBU)
Programme holder Institut Bauen und Umwelt e.V. (IBU)
Declaration number EPD-KIM-20230121-CBC1-EN
Issue date 06.06.2023
Valid to 05.06.2028
Injection moulded polypropylene products
Kima Accessories Aps
www.ibu-epd.com | https://epd-online.com
General Information
Kima Accessories Aps Injection moulded polypropylene products
Programme holder Owner of the declaration
IBU – Institut Bauen und Umwelt e.V. Kima Accessories Aps
Hegelplatz 1 Kastanievej 3
10117 Berlin 6862 Tistrup
Germany Denmark
Declaration number Declared product / declared unit
EPD-KIM-20230121-CBC1-EN 1 kilogram of a representative injection moulded polypropylene product.
This declaration is based on the product category rules: Scope:
Boards and panels made of plastic (exterior applications), This environmental product declaration describes the production of a
01.08.2021 representative product made of 100% polypropylene by injection moulding
(PCR checked and approved by the SVR) at Kima Accessories facility in Tistrup, Denmark. Hence this declaration is
a representative EPD.
It includes the following two products:
Issue date
• Storm crate
06.06.2023 • Insulation disc
The two products mentioned above are made of 100 % virgin
polypropylene by injection moulding. The data is based on data collected
Valid to at the production site and data delivered by suppliers. The data represents
the production of the period 01.07.2021 to 30.06.2022.
05.06.2028
The owner of the declaration shall be liable for the underlying information
and evidence; the IBU shall not be liable with respect to manufacturer
information, life cycle assessment data and evidences.
The EPD was created according to the specifications of EN 15804+A2. In
the following, the standard will be simplified as EN 15804.
Verification
The standard EN 15804 serves as the core PCR
Independent verification of the declaration and data according to ISO
14025:2011
Dipl.-Ing. Hans Peters
(Chairman of Institut Bauen und Umwelt e.V.) internally X externally
Dipl.-Ing. Hans Peters Dr.-Ing. Nikolay Minkov,
(Managing Director Institut Bauen und Umwelt e.V.) (Independent verifier)
1 Environmental Product Declaration - Kima Accessories Aps - Injection moulded polypropylene products
Product
• ISO 179-1
Product description/Product definition • ISO 306
This environmental product declaration covers two products • ISO 527-2
made of 100 % polypropylene (PP) by injection moulding. • ISO 1183
The product names and codes are as follows: • ISO 3302-1
• F6100 - Storm crate - 9.4 kg/pcs Constructional data
• R2022HV3 - Insulation disc - 0.008 kg/pcs
Name Value Unit
The common function of the product group is to ensure
Thickness 2 - 3 mm
environment and conditions for buildings, to prolong the lifetime
of the building. Specifically, the products ensure run-off of Gross density 0.9 - kg/m3
rainwater from the roof and into the ground, thereby, protecting 0
the building from water and moisture, as well as a environment Flexural modulus according to ISO 178 1500 MPa
for insulation materials. The products have been grouped since Melt flow rate (230C/2.16 kg) according to ISO
44 g/10min
they have the overall same function as well as the same 1133
production process.
Charpy impact strength (23C) according to ISO
7 kJ/m^2
179-1
The storm crate is burried under the ground to facilitate water
Charpy impact strength (0C) according to ISO
retention, attenuation, and infiltration. It has the following 5 kJ/m^2
179-1
dimensions: 78 x 78 x 42 cm, and a water capacity of 256 L.
Charpy impact strength (-20C) according to ISO
4 kJ/m^2
The insulation disc is used for mounting insulation to a building. 179-1
The dimensions of the insulation disc is 70 mm in diameter and Tensile stress at yield according to ISO 527-2 28 MPa
the screw hole in the middle is 6 mm. Heat deflection temperature (0.45 MPa)
100 C
according to ISO 75-2
The production of Kima Accessories injection moulded PP
Viscat softening temperature according to ISO
products have so far not been subject to EU harmonizatoin 152 C
306-1
legislation. Hence, for the use and application of the products
the respective national provisions at the place of use apply Performance data of the product with respect to its
characteristics in accordance with the relevant technical
Application provision (no CE-marking).
Storm crate:
Base materials/Ancillary materials
The storm crate is a modular cellular crate and is used in storm
water retention, attenuation and infiltration applications. The The declared product consists solely of PP (100 %
crate is designed to be simple and easily stacked together to polypropylene).
create a below ground storm water holding tank or to allow the Name Value Unit
infiltration of storm water into the ground around it. The void Polypropylene Virgin 100 %
created by the crate can fill up with storm water during heavy
This product/article/at least one partial article contains
rainfalls. The collected storm water then drains away slowly into
substances listed in the candidate list (date:12.05.2023)
the drainage.
exceeding 0.1 percentage by mass: No
Insulation disc:
The insulation disc is a polypropylene disc with spikes, that
Reference service life
helps mounting insulations, such as mineral wool, to a building.
The reference service life is not relevant for this LCA since the
The disc has four spike on one side to ensure grip on the
use stage modules B1-B7 are not included. The storm crate is
insulation material. The disc has a hole in the middle for screws
expected to have a long life time if the entire storm water
used for mounting.
system is well maintained. For this product, we expect a life
Technical Data time of 50 years, but it might be longer.
The two products covered by this environmental product
The expected lifetime of the insulation disc attached to the roof
declaration are made of 100 % virgin polypropylene C705-
construction is mounted during the construction of the building
44NAHP. Which is made for thin wall injection moulding.
or when replacing insulation. The disc is expected to be
The PP is tested in accordance with the following standards.
replaced together with the insulation material. Mineral wool has
• ISO 1133 an expected lifetime of approximately 50 years and the same is
• ISO 75-2 assumed for the insulation disc.
• ISO 178
LCA: Calculation rules
Name Value Unit
Declared Unit
Gross density 0.9 kg/m3
The declared unit is 1 kilogram of a representative injection
moulded polypropylene product. Declared unit 1 kg
Declared unit The robustness of the LCA values is judged to be good. The
production process of the two products is identical. The only
difference is the shape and weight of the two products.
2 Environmental Product Declaration - Kima Accessories Aps - Injection moulded polypropylene products
The electricity consumption was found by taking the total The deconstruction of the products is assumed to be done
electricity consumption of the production facility and dividing it manually. As a result, no processes have been assigned to
by the total production volume, as it was not possible to module C1. 95 % of the products are sold to Danish customers
measure the individual machines. The geographical the remaining 5 % is divided between other Scandinavian
representative is good, as all products are manufactured in countries (4 %) and other European countries (1 %). Hence, the
Denmark. Secondary data is used for modules A1, A2, modules transportation distance is modelled for Danish conditions. A
C and D. Collecting primary data in these stages will make the transport distance from the building to the waste processing
LCA stronger, however, it might not change the overall facilities of 50 km is assumed. End-of-life treatment of
conclusion of the LCA results. packaging material is not included as module A5 is not
declared.
System boundary
This is a cradle-to-gate EPD with modules A1-A3, C1–C4 and D Benefits and loads beyond the system boundaries -
Production stage - Module A1-A3 Module D
The production stage includes: The benefits and loads include:
• A1, raw material extraction and processing, processing • D, potential benefits from reuse, recycling and recovery
of secondary material from previous product systems, outside the scope of the study.
when applicable. • D, potential loads related to processing to reach
• A2, transport to factory gate and internal transport equivalent materials to virgin input material
• A3, manufacturing of products and packaging, as well In this case, benefits are given to the recycling of the amount of
as assembly and processing up to the end-of-waste virgin PP. The loads of the regranulation of plastic are included
state. in this study. Furthermore, a benefit is given to the exported
Wastes and losses of the manufacturing processes are energy obtained from waste incineration.
included in the processes in which they occur according to the
polluter pays principle. The construction of the manufacturing Geographic Representativeness
facility is not taken into account, however the production of Land or region, in which the declared product system is
spare parts for machinery is included in this study. The manufactured, used or handled at the end of the product´s
electricity consumption includes all activities at the lifespan: Denmark
manufacturing facility including office equipment. Input data for
the manufacturing real plant data were used.
Comparability
End-of-life stage - Module C1-C4 Basically, a comparison or an evaluation of EPD data is only
The end-of-life stage includes: possible if all the data sets to be compared were created
according to EN 15804 and the building context, respectively
• C1, deconstruction and demolition
the product-specific characteristics of performance, are taken
• C2, transport to waste processing
into account. The system model EN15804 - cut-off available in
• C3, waste processing for reuse, recovery and/or
the LCI database Ecoinvent v. 3.9 is used in this EPD.
recycling
• C4, disposal
LCA: Scenarios and additional technical information
Name Value Unit
Characteristic product properties of biogenic carbon
Packaging waste for recycling (Cardboard) 0.03 kg
The biogenic carbon content quantifies the amount of biogenic
Packaging waste for recycling (Wood pallet) 0.02 kg
carbon in a construction product leaving the factory gate. Both
the biogenic content of the product and the accompanying Packaging waste for incineration (Plastic film) 0.002 kg
packaging is declared. Packaging waste for incineration (Tape) 0.006 kg
Note: 1 kg of biogenic carbon is equivalent to 44/12 kg of CO . End of life (C1-C4)
2
Name Value Unit
Information on describing the biogenic Carbon Content at
factory gate Collected separately 0.9 kg
Collected as mixed construction waste 0.1 kg
Name ValueUnit
Recycling PP 0.9 kg
kg
Biogenic carbon content in product -
C Energy recovery PP 0.1 kg
Biogenic carbon content in accompanying kg
0.06 Reuse, recovery and/or recycling potentials (D), relevant
packaging Cardboard C
scenario information
Biogenic carbon content in accompanying kg
0.04 The following values in the table are amounts contributing to
packaging Wood C
the loads and benefits included in module D.
Name Value Unit
The following technical scenario information covers the disposal
Recycling of PP from module C3 0.9 kg
of the accompanying packaging material of A3, on the
Incineration of PP from module C3 0.1 kg
construction site as module A5 is not declared in this EPD.
Credits are only given to the net amount leaving the product
Installation into the building (A5)
system that has passed the end-of-waste state.
In the LCA calculation loads related to obtaining equivalent
functions as the original virgin material are included as well as
benefits of avoided production of the given virgin material.
3 Environmental Product Declaration - Kima Accessories Aps - Injection moulded polypropylene products
LCA: Results
The following table shows the LCA results obtained in this study.
For calculation of the results, characterization was used on a model created of individual inputs from different LCIA methods to comply
with EN15804+A2 which is yet to be fully implemented in the SimaPro software. As a result, the LCIA has been calculated in Excel
using the following methods from EcoInvent v.3.9:
• EF v.3.1 EN 15804
• EN 15804 inventory indicators according to ISO 21930
The additional indicators are retrieved by using ecoinvent cumulative LCIA results for the system model EN15804, cut-off. It follows ISO
21930; hence the results include all the foreground and background processes.
C1 is declared as 0, since manual deconstruction is assumed.
C4 is declared as 0, since no landfilling is assumed in the end-of-life stage.
The estimated impact results are only relative statements which do not indicate the endpoints of the impact categories, exceeding
threshold values, safety margins or risks.
DESCRIPTION OF THE SYSTEM BOUNDARY (X = INCLUDED IN LCA; ND = MODULE OR INDICATOR NOT DECLARED; MNR =
MODULE NOT RELEVANT)
Benefits and
Construction loads beyond
Product stage Use stage End-of-life stage
process stage the system
boundaries
la ire ta m w a Ry lp p u s tro p s n a rT g n iru tc a fu n a M e h t m o rf tro p s n a rTe tis e h t o t e ta g y lb m e s s A e s U e c n a n e tn ia M ria p e R tn e m e c a lp e R tn e m h s ib ru fe R y g re n e la n o ita re p Oe s u re ta w la n o ita re p Oe s u n o itc u rts n o c -e Dn o itilo m e d tro p s n a rT g n is s e c o rp e ts a W la s o p s iD -e s u e R-y re v o c e R-g n ilc y c e Rla itn e to p
A1 A2 A3 A4 A5 B1 B2 B3 B4 B5 B6 B7 C1 C2 C3 C4 D
X X X MND MND MND MND MNR MNR MNR MND MND X X X X X
RESULTS OF THE LCA - ENVIRONMENTAL IMPACT according to EN 15804+A2: 1 kg injection moulded polypropylene
product
Parameter Unit A1-A3 C1 C2 C3 C4 D
Global Warming Potential total (GWP-total) kg CO 2 eq 3.15E+00 0 7.39E-03 7.27E-01 0 -1.71E+00
Global Warming Potential fossil fuels (GWP-fossil) kg CO 2 eq 3.53E+00 0 7.38E-03 -1.73E-04 0 -1.7E+00
Global Warming Potential biogenic (GWP-biogenic) kg CO 2 eq -3.81E-01 0 5.93E-06 1.4E-04 0 -9.37E-03
Global Warming Potential luluc (GWP-luluc) kg CO 2 eq 2.98E-03 0 3.68E-06 7.33E-09 0 -4.16E-04
Depletion potential of the stratospheric ozone layer (ODP) kg CFC11 eq 4.36E-08 0 1.64E-10 1.38E-03 0 -8.19E-09
Acidification potential of land and water (AP) mol H+ eq 1.25E-02 0 1.69E-05 1.43E-04 0 -5.97E-03
Eutrophication potential aquatic freshwater (EP-freshwater) kg P eq 8.02E-04 0 5.43E-07 4.12E-04 0 -1.93E-04
Eutrophication potential aquatic marine (EP-marine) kg N eq 2.47E-03 0 4.39E-06 3.3E-03 0 -1.05E-03
Eutrophication potential terrestrial (EP-terrestrial) mol N eq 2.52E-02 0 4.46E-05 9.88E-04 0 -1.11E-02
Formation potential of tropospheric ozone photochemical oxidants kg NMVOC
1.05E-02 0 2.67E-05 1.17E-06 0 -5.54E-03
(POCP) eq
Abiotic depletion potential for non fossil resources (ADPE) kg Sb eq 1.49E-05 0 2.41E-08 5.88E+00 0 -7.5E-06
Abiotic depletion potential for fossil resources (ADPF) MJ 9.95E+01 0 1.08E-01 6.97E-02 0 -6.56E+01
m3 world eq
Water use (WDP) 1.02E+00 0 5.54E-04 2.76E-01 0 -6.56E-01
deprived
RESULTS OF THE LCA - INDICATORS TO DESCRIBE RESOURCE USE according to EN 15804+A2: 1 kg injection moulded
polypropylene product
Parameter Unit A1-A3 C1 C2 C3 C4 D
Renewable primary energy as energy carrier (PERE) MJ 7.85E+00 0 1.73E-03 0 0 -9.32E-01
Renewable primary energy resources as material utilization
MJ 2.86E+00 0 0 2.76E-01 0 0
(PERM)
Total use of renewable primary energy resources (PERT) MJ 1.07E+01 0 1.73E-03 -3.55E+01 0 -9.32E-01
Non renewable primary energy as energy carrier (PENRE) MJ 6.62E+01 0 1.08E-01 4.14E+01 0 -3.61E+01
Non renewable primary energy as material utilization (PENRM) MJ 3.33E+01 0 0 5.88E+00 0 -2.95E+01
Total use of non renewable primary energy resources (PENRT) MJ 9.95E+01 0 1.08E-01 3.56E-03 0 -6.56E+01
Use of secondary material (SM) kg 2.15E-02 0 4.88E-05 2.77E-05 0 -2.5E-03
Use of renewable secondary fuels (RSF) MJ 4.85E-02 0 5.97E-07 0 0 -2.58E-05
Use of non renewable secondary fuels (NRSF) MJ 0 0 0 7.2E-03 0 0
Use of net fresh water (FW) m3 4.55E-02 0 1.39E-05 3.63E-02 0 -1.64E-02
RESULTS OF THE LCA – WASTE CATEGORIES AND OUTPUT FLOWS according to EN 15804+A2:
1 kg injection moulded polypropylene product
Parameter Unit A1-A3 C1 C2 C3 C4 D
Hazardous waste disposed (HWD) kg 1.48E-01 0 7.34E-05 7.97E-01 0 -2.17E-02
Non hazardous waste disposed (NHWD) kg 3.69E+00 0 2.3E-03 4.12E-06 0 -8.13E-01
4 Environmental Product Declaration - Kima Accessories Aps - Injection moulded polypropylene products
Radioactive waste disposed (RWD) kg 2.36E-05 0 9.03E-09 0 0 -5.25E-06
Components for re-use (CRU) kg 0 0 0 8.17E-01 0 0
Materials for recycling (MFR) kg 1.28E-03 0 8.25E-07 3.87E-07 0 -2.2E-04
Materials for energy recovery (MER) kg 1.77E-06 0 4.91E-09 1.03E-01 0 -5.12E-07
Exported electrical energy (EEE) MJ 4.07E-01 0 1.83E-05 2.99E-03 0 -1.43E-02
Exported thermal energy (EET) MJ 2E-02 0 4.77E-05 1.11E-08 0 -4.98E-03
RESULTS OF THE LCA – additional impact categories according to EN 15804+A2-optional:
1 kg injection moulded polypropylene product
Parameter Unit A1-A3 C1 C2 C3 C4 D
Disease
Incidence of disease due to PM emissions (PM) 1.21E-07 0 5.98E-10 8.09E-02 0 -6.47E-08
incidence
Human exposure efficiency relative to U235 (IR) kBq U235 eq 4.57E-01 0 1.52E-04 1.66E+00 0 -9.11E-02
Comparative toxic unit for ecosystems (ETP-fw) CTUe 6.92E+00 0 5.27E-02 2.92E-10 0 -1.6E+00
Comparative toxic unit for humans (carcinogenic) (HTP-c) CTUh 1.69E-09 0 3.5E-12 4.89E-09 0 -4.35E-10
Comparative toxic unit for humans (noncarcinogenic) (HTP-nc) CTUh 3.09E-08 0 7.65E-11 1.78E+00 0 -8.63E-09
Soil quality index (SQP) SQP 5.07E+01 0 8.08E-02 ND 0 -1.37E+00
Disclaimer 1 – for the indicator 'Potential Human exposure efficiency relative to U235'.This impact category deals mainly with the
eventual impact of low-dose ionizing radiation on human health of the nuclear fuel cycle. It does not consider effects due to possible
nuclear accidents, occupational exposure or radioactive waste disposal in underground facilities. Potential ionizing radiation from the
soil, radon and from some construction materials is also not measured by this indicator.
Disclaimer 2 – for the indicators 'abiotic depletion potential for non-fossil resources', 'abiotic depletion potential for fossil resources',
'water (user) deprivation potential, deprivation-weighted water consumption', 'potential comparative toxic unit for ecosystems', 'potential
comparative toxic unit for humans – cancerogenic', 'Potential comparative toxic unit for humans - not cancerogenic', 'potential soil
quality index'. The results of this environmental impact indicator shall be used with care as the uncertainties on these results are high
as there is limited experience with the indicator.
References
Standards for Products Moulded in Solid Rubber
EN 15804
EN 15804:2012+A2:2019+AC:2021, Sustainability of ISO 14025
construction works — Environmental Product Declarations — EN ISO 14025:2011, Environmental labels and declarations —
Core rules for the product category of construction products. Type III environmental declarations — Principles and
procedures.
ISO 75-2:2013
Plastics — Determination of temperature of deflection under ISO 14040
load — Part 2: Plastics and ebonite ISO 14040:2006, Environmental management –Life cycle
assessment - Principles and framework;English version
ISO 178
ISO 178:2019, Plastics – Determination
of flexural properties ISO 14044
ISO 14044:2006, Environment Management – LifeCycle
ISO 179-1 Assessment – Requirements and Instructions;English version
ISO 179-1:2010, Plastics – Determination EN ISO 14044:2006.
of Charpy impact properties— Part 1: Non-instrumented impact
test Further references
ISO 306 ECHA candidate list
ISO 306:2004, Plastics – Candidate List of substances of very high concern for
Thermoplastics materials- Determination of Vicat softening Authorisation
temperature https://echa.europa.eu/candidate-list-table [Accessed 25-05-
2023].
ISO 527-2
ISO 527-2:2012, EcoInvent 3.9
Plastics — Determination of tensile properties — Part 2: Test EcoInvent database version 3.9, cut-off, EN15804model. LCIA
conditions for moulding and extrusion plastics methodology EF v3.1 EN15804.Wernet, G., Bauer, C.,
Steubing, B., Reinhard, J., Moreno-Ruiz, E., and Weidema, B.,
ISO 1133 2016. The ecoinvent database version 3 (part I): overview and
ISO 1133:2011, Plastics – Determination of the melt mass-flow methodology. The International Journal of Life Cycle
rate and melt volume-flow rate of Assessment, [online] 21(9), pp.1218–1230. Available at:
thermoplastics [Accessed 06-01-2023].
ISO 1183 IBU 2018
ISO 1183:2019, Plastics – Methods for Product Category Rules for Building-Related Products
determining the density of non-cellular plastics and Services, Part A: Calculation Rules for the Life
Cycle Assessment and Requirements on the Project
ISO 3302-1 Report, Version 1.3
ISO 3302-1:2014, Classes and Tolerances
5 Environmental Product Declaration - Kima Accessories Aps - Injection moulded polypropylene products
IBU 2021 Services, Part B: Requirements on the EPD for Boards and
Institut Bauen und Umwelt e.V.: General Instructions for the panels made of plastic (exterior applications), Version 1.0
EPD programme of Institut Bauen und Umwelt e.V., Version
2.0, Berlin: Institut Bauen und Umwelt e.V., 2021 www.ibu- SimaPro 2023
epd.com Pré Sustainability,
LCA software SimaPro version 9.5.
IBU 2023
PCR Guidance-Text for Building-Related Products and
6 Environmental Product Declaration - Kima Accessories Aps - Injection moulded polypropylene products
Publisher
Institut Bauen und Umwelt e.V. +49 (0)30 3087748- 0
Hegelplatz 1 info@ibu-epd.com
10117 Berlin www.ibu-epd.com
Germany
Programme holder
Institut Bauen und Umwelt e.V. +49 (0)30 3087748- 0
Hegelplatz 1 info@ibu-epd.com
10117 Berlin www.ibu-epd.com
Germany
Author of the Life Cycle Assessment
Viegand Maagøe +4533349000
Nørre Farigmagsgade 37 info@viegandmaagoe.dk
1364 Copenhagen www.viegandmaagoe.dk/en
Denmark
Owner of the Declaration
Kima Accessories Aps +4575330800
Kastanievej 3 mail@kimaroof.dk
6862 Tistrup www.kimaroof.dk
Denmark
7 Environmental Product Declaration - Kima Accessories Aps - Injection moulded polypropylene products
