ENVIRONMENTAL PRODUCT DECLARATION
as per ISO 14025 and EN 15804+A1
Owner of the Declaration Stiferite
Publisher Institut Bauen und Umwelt e.V. (IBU)
Programme holder Institut Bauen und Umwelt e.V. (IBU)
Declaration number EPD-STF-20200236-CBA3-EN
Issue date 18.12.2020
Valid to 17.12.2025
Stiferite Isocanale A6B average thickness panel
Stiferite
www.ibu-epd.com | https://epd-online.com
General Information
Stiferite Stiferite Isocanale A6B average thickness panel
Programme holder Owner of the declaration
IBU – Institut Bauen und Umwelt e.V. Stiferite
Hegelplatz 1 Viale Navigazione Interna 54
10117 Berlin 35129 Padova
Germany Italy
Declaration number Declared product / declared unit
EPD-STF-20200236-CBA3-EN STIFERITE ISOCANALE A6B expanded rigid polyurethane foam, covered
on both sides by embossed antibacterial aluminum of 60 µm thickness,
and produced by Stiferite. The EPD applies to 1 m2 of an average
thickness of 20 mm PUR sandwich board, i.e. 0.020 m3, with an average
density between foam and facing of 53 kg/m3.
This declaration is based on the product category rules: Scope:
Insulating materials made of foam plastics, 01.08.2021 Stiferite produces STIFERITE ISOCANALE A6B that is a high-performance
(PCR checked and approved by the SVR) insulation board manufactured from closed cell expanded rigid
polyurethane foam, covered on both sides by embossed antibacterial
aluminum of 60 my thickness. The data have been provided by the only
Issue date Stiferite factory that were located in Padova (Italy) for the year 2015.
The owner of the declaration shall be liable for the underlying information
18.12.2020
and evidence; the IBU shall not be liable with respect to manufacturer
information, life cycle assessment data and evidences.
Valid to
The EPD was created according to the specifications of EN 15804+A1. In
17.12.2025 the following, the standard will be simplified as EN 15804.
Verification
The standard EN 15804 serves as the core PCR
Independent verification of the declaration and data according to ISO
14025:2011
internally X externally
Dipl.-Ing. Hans Peters
(Chairman of Institut Bauen und Umwelt e.V.)
Dipl.-Ing. Hans Peters Prof. Dr. Birgit Grahl,
(Managing Director Institut Bauen und Umwelt e.V.) (Independent verifier)
1 Environmental Product Declaration - Stiferite - Stiferite Isocanale A6B average thickness panel
Product
This provides a thermal resistance R = 0.952 m² k/W.
Product description/Product definition
STIFERITE's thermoinsulation panels are mainly used in the The LCI data used in this report refer to an average product
building/construction sector and that of industrial insulation. having an average thickness (materials in the recipes of
different thicknesses are weighted according to the relative
The panels are made of thermo-setting closed cells production in square meters). The type of declaration is 1 c -
polyurethane foam (PU) supplied with various types of flexible declaration of an average product from a manufacturer's plant.
facers on both sides of the panel. The nature/type of facer
contributes to the performance characteristics of the product Product according to CPR, based on a EN performance data of
and its application. the product in accordance with declaration of performance with
respect to its essential characteristics according to /EN
Expanded rigid polyurethane foam is distinguished by its good 13165:2012+A2:2016 Thermal insulation products for building -
thermo insulation performance, mechanical resistance, factory made rigid polyurethane foam (PU) products -
workability, lightness, and durability. specification/ and CE mark.
The performance of STIFERITE's panels is determined based Base materials/Ancillary materials
on the European norm EN 13165:2012+A2:2016 Thermal Core material (about 68.4% of the weight of the declared unit):
insulation products for buildings - Factory made rigid Closed-cell Polyiso (PIR) rigid foam made from MDI (50-65%),
polyurethane foam (PU) products - Specification. polyols (20-30%), pentane (4-5%) and additives (4-7%).
This EPD refers to STIFERITE's ISOCANALE A6B average Facing (about 31.6% of the weight of the declared unit):
thickness panel, made of an insulation component in aluminum of 60 my thickness consisting of aluminum (99-97%)
polyurethane foam using blowing agent Pentane-based, and lacquere (1-3%).
covered on both sides by embossed antibacterial aluminum of
60 µm thickness. The PU board for insulation:
• This product/article/at least one partial article contains
The panel is produced with the standard dimensions of 1200 x
substances listed in the candidate list (date: 17.11.2020)
4000 mm and with straight finished edges.
exceeding 0.1 percentage by mass: no
• This product/article/at least one partial article doesn't
Upon request and for minimum quantities, the panels may be
contain other CMR substances in categories 1A or 1B
produced in various dimensions. STIFERITE ISOCANALE A6B
which are not on the candidate list, exceeding 0.1
panel is produced by a certified company with systems: ISO
percentage by mass: no
9001, OHSAS 45001, ISO 14001 in its entire line of products.
• Biocide products were added to this construction
For the placing on the market in the EuropeanUnion/European
product or it has been treated with biocide products (this
Free Trade Association (EU/EFTA) (with the exception of
then concerns a treated product as defined by the (EU)
Switzerland) th Regulation (EU) No 30572011 applies. The
Ordinance on Biocide Products No. 528/2012): no
insulation products need a Declaration of Performance taking
Additional declaration according to quoted law: The product is
into consideration the EN 13165:2012+A2:2016 Thermal
compliant with all requirements indicated at Additional
insulation products for buildings — Factory made rigid
declaration according to quoted law: The product is compliant
polyurethane foam (PU) products — Specification and the CE-
with all requirements indicated in chapter 2.5.7 'Isolanti termici
marking. For the use and application of the product the
ed acustici' of the n.256 D.L. of the 23th June 2022 (CAM
respective national provisions at the place of use apply.
EDILIZIA):
Application • Any blowing agent with Ozone depletion potential >0 is
The STIFERITE ISOCANALE A6B panel is suited for the not used in production
construction of pre-insulated heating and ventilation ducts. • Any substances of Very High Concern-SVHC in
concentration of more than 0,1 %w are not used in
Technical Data production (REACH n. 1907/2006). Any specific
For the insulation products the data of their Declaration of authorizations for use are eserved provided for by the
Performance (DoP) apply. In this Life Cycle Assessment, a PU same Regulation for the substances included in Annex
insulation board with the following properties has been XIV and specifications restrictions set out in Annex XVII
regarded: of the Regulation.
• Catalysts lead-based are not used in production
Constructional data
• Flame retardants used in production (belonging to the
Name Value Unit
Organophosphorus class) are not banned by any
Gross density 53 kg/m3 national or European regulation
Declared Average Thermal conductivity λi acc. • According to the raw materials declarations of suppliers
0.021 W/mK
to /EN 13165/ the minimum amount of recycled raw materials based
on the insulation board (PU foam and facers) weight is 3
Water absorption by total immersion acc. to /EN Vol.-
< 1 %w and the minimum amount of recycled raw materials
12087/ %
based on the PU insulation foam weight is 4 %w (note:
Water absorption by partial immersion acc. to
< 0.1 kg/m² this information is not explicitly considered in the LCA
/EN 1609/
and not included in the EPD tables that only refer to
Water vapour diffusion resistance factor μ acc.
endless recycling content in the foreground system).
to /EN 12086/
Euroclass reaction to fire - Stiferite Duct acc. to Reference service life
B s1 d0
/EN 11925/ The durability of insulation panels is normally at least as long as
the lifetime of the building in which it is used. The experimental
2 Environmental Product Declaration - Stiferite - Stiferite Isocanale A6B average thickness panel
data show that the reference life is longer than 50 years, Clima 2019 .
LCA: Calculation rules
gate with options). It also includes the transport to the
Declared Unit construction site, the installation and the end-of-life stage of the
The declared unit is 1 m² with with an average thickness of 20 used PU thermal insulation board. The life cycle is split into the
mm, e. g. 0.02 m³. Corresponding conversion factors are listed following individual phases:
in the table below. A1 - Raw material formulation
Declared unit A2 - Raw material transport
A3 - Production of the insulation board and packaging material
Name Value Unit
A4 - Transport to the construction site
Declared unit 1 m2 A5 - Emissions and cutting losses during installation and
Gross density 53 kg/m3 packaging disposal
Volume 0.02 m³ C2 - Transport to end of life
C3/C4 - End-of-Life: waste management (thermal recovery,
Grammage 106 kg/m2
landfill)
Declared average thermal conductivity λi 0.021 W/mK D - Benefits and loads beyond system boundary
Layer thickness 0.02 m
Geographic Representativeness
Conversion factor to 1 kg 1.06 kg/m²
Land or region, in which the declared product system is
Weight of declared unit 1.06 kg/m²
manufactured, used or handled at the end of the product´s
The LCI data used in this report refer to an average product lifespan: Italy
having an average thickness (materials in the recipes of
different thicknesses are weighted according to the relative
production in square meters). The type of declaration is 1 c - Comparability
declaration of an average product from a manufacturer's plant. Basically, a comparison or an evaluation of EPD data is only
possible if all the data sets to be compared were created
according to EN 15804 and the building context, respectively
the product-specific characteristics of performance, are taken
System boundary into account. For life cycle modelling of the considered
This life cycle assessment for the production of the products, the GaBi 9 2020 has been used.
polyurethane insulation board considers the life cycle from the
supply of raw materials to the manufacturer´s gate (cradle-to-
LCA: Scenarios and additional technical information
The results for the end-of-life are declared for the 2 different
scenarios:
Name Value Unit
Transport to the building site (A4) Scenario No 1: Material Incineration 100 %
The distances calculated are weighted average distances Scenario No 2: Landfill 100 %
according to the overall sales distribution; such distribution is
C4: Disposal scenarios used is divided into the 2
considered similar for all Stiferite products.
sub-scenarios:
Name ValueUnit
1) Incineration 100% (C4/1)
Truck with a capacity of 17.3 tons 271 km 2) Landfilling 100% (C4/2)
Ferry with a capacity of 1200-10000 dwt payload
144 km
capacity D: Benefits and loads beyond system boundary is divided into
Ship with a capacity of 27500 dwt payload capacity the 2 sub-scenarios:
tons 11000 km 1) Incineration 100% (D1)
2) Landfilling 100% (D2)
Plane with a capacity of 22 ton 0 km
Installation into the building (A5) Reuse, recovery and/or recycling potentials (D), relevant
Name Value Unit scenario information
Material loss 0.0212 kg Name Value Unit
VOC in the air Pentane 1.27E-06 kg Module D includes credits from recycling materials of insulation
panels and packaging, energy credits from thermal recovery of
the packaging. The results are declared for the same 3 different
End of life (C1-C4)
scenarios described above.
3 Environmental Product Declaration - Stiferite - Stiferite Isocanale A6B average thickness panel
LCA: Results
The tables below show the results of the LCA. Basic information on all declared modules provides chapter 4.
There are two scenarios for the end-of-life (C3, C4 and D) analyzed: Scenario 1 considers 100% incineration, Scenario 2 considers
100% landfill disposal.
For (SM, RSF, NRSF, CRU) indicators only the foreground system is considered.
DESCRIPTION OF THE SYSTEM BOUNDARY (X = INCLUDED IN LCA; MND = MODULE NOT DECLARED; MNR = MODULE NOT
RELEVANT)
Benefits and
Construction loads beyond
Product stage Use stage End-of-life stage
process stage the system
boundaries
la ire ta m w a Ry lp p u s tro p s n a rT g n iru tc a fu n a M e h t m o rf tro p s n a rTe tis e h t o t e ta g y lb m e s s A e s U e c n a n e tn ia M ria p e R tn e m e c a lp e R tn e m h s ib ru fe R y g re n e la n o ita re p Oe s u re ta w la n o ita re p Oe s u n o itc u rts n o c -e Dn o itilo m e d tro p s n a rT g n is s e c o rp e ts a W la s o p s iD -e s u e R-y re v o c e R-g n ilc y c e Rla itn e to p
A1 A2 A3 A4 A5 B1 B2 B3 B4 B5 B6 B7 C1 C2 C3 C4 D
X X X X X MND MND MNR MNR MNR MND MND MND X X X X
RESULTS OF THE LCA - ENVIRONMENTAL IMPACT according to EN 15804+A1: 1 m² Stiferite A6B average thickness panel
Parameter Unit A1-A3 A4 A5 C2 C3/1 C3/2 C4/1 C4/2 D/1 D/2
GWP kg CO 2 eq 5.65E+00 2.43E-02 2.05E-01 4.89E-03 0 0 1.67E+00 4.82E-02 -7.91E-01 9.5E-02
ODP kg CFC11 eq 3.18E-06 1.54E-13 6.32E-08 3.53E-14 0 0 3.64E-11 1.96E-11 -5.22E-10 -1.24E-11
AP kg SO 2 eq 2.03E-02 2.2E-04 4.5E-04 1.22E-05 0 0 8.27E-04 1.82E-04 -2.24E-03 -1.53E-04
EP kg PO 43 eq 1.67E-03 2.87E-05 6.07E-05 2.84E-06 0 0 1.87E-04 2.16E-05 -2.37E-04 -4.42E-05
POCP kg Ethen eq 3.23E-03 -2.61E-06 7.51E-05 -3.37E-06 0 0 5.81E-05 1.54E-05 -1.91E-04 -2.83E-05
ADPE kg Sb eq 6.84E-06 1.53E-09 1.44E-07 3.65E-10 0 0 4.8E-08 1.63E-08 -2.91E-07 -5.29E-08
ADPF MJ 8.9E+01 3.26E-01 2.39E+00 6.73E-02 0 0 1.17E+00 5.28E-01 -1.12E+01 -7.06E-01
GWP = Global warming potential; ODP = Depletion potential of the stratospheric ozone layer; AP = Acidification potential of land and water; EP =
Eutrophication potential; POCP = Formation potential of tropospheric ozone photochemical oxidants; ADPE = Abiotic depletion potential for non-fossil
resources; ADPF = Abiotic depletion potential for fossil resources
RESULTS OF THE LCA - INDICATORS TO DESCRIBE RESOURCE USE according to EN 15804+A1: 1 m² Stiferite A6B average
thickness panel
Parameter Unit A1-A3 A4 A5 C2 C3/1 C3/2 C4/1 C4/2 D/1 D/2
PERE MJ 2.22E+01 IND 1.87E+00 IND IND IND 2.72E-01 IND IND IND
PERM MJ 1.36E+00 IND -1.36E+00 IND IND IND 0 IND IND IND
PERT MJ 2.36E+01 1.48E-02 5.12E-01 3.88E-03 0 0 2.72E-01 1.61E-01 -6.11E+00 -2.6E+00
PENRE MJ 6.99E+01 IND 1.52E+00 IND IND IND 2.92E+01 IND IND IND
PENRM MJ 2.86E+01 IND -9.43E-01 IND IND IND -2.77E+01 IND IND IND
PENRT MJ 9.85E+01 3.27E-01 5.81E-01 6.76E-02 0 0 1.51E+00 7.17E-01 -1.6E+01 -7.89E-01
SM kg 0 0 0 0 0 0 0 0 0 0
RSF MJ 0 0 0 0 0 0 0 0 0 0
NRSF MJ 0 0 0 0 0 0 0 0 0 0
FW m3 6.12E-02 3.65E-05 1.76E-03 9.59E-06 0 0 4.93E-03 2.55E-04 -5.74E-03 -3.26E-04
PERE = Use of renewable primary energy excluding renewable primary energy resources used as raw materials; PERM = Use of renewable primary
energy resources used as raw materials; PERT = Total use of renewable primary energy resources; PENRE = Use of non-renewable primary energy
excluding non-renewable primary energy resources used as raw materials; PENRM = Use of non-renewable primary energy resources used as raw
materials; PENRT = Total use of non-renewable primary energy resources; SM = Use of secondary material; RSF = Use of renewable secondary fuels;
NRSF = Use of non-renewable secondary fuels; FW = Use of net fresh water
RESULTS OF THE LCA – WASTE CATEGORIES AND OUTPUT FLOWS according to EN 15804+A1:
1 m² Stiferite A6B average thickness panel
Parameter Unit A1-A3 A4 A5 C2 C3/1 C3/2 C4/1 C4/2 D/1 D/2
HWD kg 7.51E-06 1.91E-08 1.61E-07 5.06E-09 0 0 4.82E-09 5.58E-09 -9.36E-08 -8.52E-08
NHWD kg 9.03E-01 2.23E-05 5.85E-02 5.83E-06 0 0 1.53E-01 1.06E+00 -8.95E-03 -1.08E-03
RWD kg 3.8E-03 6.33E-07 6.39E-05 1.45E-07 0 0 1.39E-04 7.54E-05 -1.92E-03 -3.32E-05
CRU kg 2.55E-03 0 5.1E-05 0 0 0 0 0 0 0
MFR kg 0 0 8.34E-02 0 0 0 0 0 0 0
MER kg 0 0 1.76E-02 0 0 0 1.06E+00 0 0 0
EEE MJ 0 0 5.14E-02 0 0 0 5.54E+00 0 0 0
EET MJ 0 0 1.05E-01 0 0 0 2.41E+00 0 0 0
HWD = Hazardous waste disposed; NHWD = Non-hazardous waste disposed; RWD = Radioactive waste disposed; CRU = Components for re-use;
MFR = Materials for recycling; MER = Materials for energy recovery; EEE = Exported electrical energy; EET = Exported thermal energy
Disclaimer 1 – for the indicator 'Potential Human exposure efficiency relative to U235'. This impact category deals mainly with the
4 Environmental Product Declaration - Stiferite - Stiferite Isocanale A6B average thickness panel
eventual impact of low-dose ionizing radiation on human health of the nuclear fuel cycle. It does not consider effects due to possible
nuclear accidents, occupational exposure or radioactive waste disposal in underground facilities. Potential ionizing radiation from the
soil, radon and from some construction materials is also not measured by this indicator.
Disclaimer 2 – for the indicators 'abiotic depletion potential for non-fossil resources', 'abiotic depletion potential for fossil resources',
'water (user) deprivation potential, deprivation-weighted water consumption', 'potential comparative toxic unit for ecosystems', 'potential
comparative toxic unit for humans – cancerogenic', 'Potential comparative toxic unit for humans - not cancerogenic', 'potential soil
quality index'. The results of this environmental impact indicator shall be used with care as the uncertainties on these results are high
as there is limited experience with the indicator.
References
Standards
BNB
EN 15804 Bewertungssystem Nachhaltiges Bauen (en: assessment
EN 15804:2012-04+A1 2013, Sustainability of construction system sustainable building)
works — Environmental Product Declarations — Core rules for https://www.bbsr.bund.de/BBSR/EN/RP/FutureBuilding/2SustainableBuildingQuality/2009/ServiceLife/01_Start_dossier.html?
the product category of construction products. n=391866&notFirst=true&docId=390900
ISO 14025 Candidate List
DIN EN ISO 14025:2011-10, Environmental labels and https://echa.europa.eu/it/candidate-list-table (date 17.11.2020)
declarations — Type III environmental declarations —
Principles and procedures. Clima 2019
Clima 2019 PaperPolyurethane 'Environmental Impacts for a
IBU 2016 Polyurethane Panel' E. Guolo, F. Cappelletti, P. Romagnoni, F.
Institut Bauen und Umwelt e.V.: General Programme Raggiotto
Instructions for the Preparation of EPDs at the Institut Bauen
und Umwelt e.V. Version 1., Berlin: Institut Bauen und Umwelt GaBi 9 2020
e.V., 2016. GaBi 8: Documentation of GaBi 8: Software-System and
www.ibu-epd.com Database for Life Cycle Engineering. Copyright, TM. Stuttgart,
Leinfelden-Echterdingen, 1992-2020
EN 13165 http://www.gabi-software.com
EN 13165:2012+A2:2016 Thermal insulation products for
buildings - Factory made rigid polyurethane foam (PU) PANGPP 2017
products - Specification Piano d' Azione Nazionale sul Green Public Procurement
(PANGPP) – Gazzetta Ufficiale della Repubblica Italiana, Serie
EN 826 Generale n.17, 11-10-2017,
EN 826:2013 Determination of Compression Behavior of http://www.minambiente.it/sites/default/files/archivio/allegati/GPP/GPP_CAM_Edilizia.pdf
Thermal Insulation Products
ISO 9001
EN 1607 ISO 9001:2015 Quality management
EN 1607:2013 Thermal insulating products for building
applications. Determination of tensile strength perpendicular to ISO 14001
faces ISO 14001: 2015 Environmental management systems
EN 12087 ISO 45001
EN 12087:2013 Thermal insulating products for building ISO 45001: 2018 Occupational health and safety management
applications. Determination of long term water absorption by systems
immersion.
PCR Part A
EN 1609 Product Category Rules for Building-Related Products and
EN 1609: Thermal insulating products for building applications. Services. Part A: Calculation Rules for the Life Cycle
Determination of short term water absorption by partial Assessment and Requirements on the Background Report.
immersion. Version 06.2017
EN 12086 PCR Part B
EN 12086: 2013 Thermal insulating products for building PCR Guidance-Texts for Building-Related Products and
applications. Determination of water vapour transmission Services; Part B: Requirements on the EPD for Insulating
properties. materials made of foam plastics; Institute Construction and
Environment e.V. (IBU). Version 06.2017
EN 11925 https://epd-online.com
EN 11925:2010 Reaction to fire tests. Ignitability of products
subjected to direct impingement of flame. Single-flame source REACH
test. REACH Registration, Evaluation, Authorization and Restriction
of Chemical, 2007
Further References
5 Environmental Product Declaration - Stiferite - Stiferite Isocanale A6B average thickness panel
Publisher
Institut Bauen und Umwelt e.V. +49 (0)30 3087748- 0
Hegelplatz 1 info@ibu-epd.com
10117 Berlin www.ibu-epd.com
Germany
Programme holder
Institut Bauen und Umwelt e.V. +49 (0)30 3087748- 0
Hegelplatz 1 info@ibu-epd.com
10117 Berlin www.ibu-epd.com
Germany
Author of the Life Cycle Assessment
thinkstep Italy +39 0544 467132
Via Bovini 43 info@thinkstep.com
48123 Ravenna www.thinkstep.com
Italy
Owner of the Declaration
Stiferite +39 049 8997911
Viale Navigazione Interna 54 info@stiferite.com
35129 Padova www.stiferite.com
Italy
6 Environmental Product Declaration - Stiferite - Stiferite Isocanale A6B average thickness panel
