ENVIRONMENTAL PRODUCT DECLARATION
as per ISO 14025 and EN 15804+A2
Owner of the Declaration Stiferite
Publisher Institut Bauen und Umwelt e.V. (IBU)
Programme holder Institut Bauen und Umwelt e.V. (IBU)
Declaration number EPD-STF-20220335-CBC2-EN
Issue date 16.02.2023
Valid to 15.02.2028
Stiferite Isocanale Ai8 average thick panel
Stiferite
www.ibu-epd.com | https://epd-online.com
General Information
Stiferite Stiferite Isocanale Ai8 average thick panel
Programme holder Owner of the declaration
IBU – Institut Bauen und Umwelt e.V. Stiferite
Hegelplatz 1 Viale Navigazione Interna 54
10117 Berlin 35129 Padova
Germany Italy
Declaration number Declared product / declared unit
EPD-STF-20220335-CBC2-EN Stiferite Isocanale Ai8 expanded rigid polyurethane foam, covered on both
sides by embossed aluminium of 80 my thickness, and produced by
Stiferite. The EPD applies to 1 m2 of 20.0 mm thick PUR sandwich board,
i.e. 0.0200 m3, with an average density between foam and facing of 47.6
kg/m3.
This declaration is based on the product category rules: Scope:
Insulating materials made of foam plastics, 01.08.2021 Stiferite produces Stiferite Isocanale AI8 that is a high-performance
(PCR checked and approved by the SVR) insulation board manufactured from closed cell expanded rigid
polyurethane foam, covered on both sides by embossed aluminium of 80
my thickness. The data have been provided by the only Stiferite factory
Issue date that is located in Padova (Italy) for the year 2021 and sold worldwide.
The owner of the declaration shall be liable for the underlying information
16.02.2023
and evidence; the IBU shall not be liable with respect to manufacturer
information, life cycle assessment data and evidences.
Valid to
The EPD was created according to the specifications of EN 15804+A2. In
15.02.2028 the following, the standard will be simplified as EN 15804.
Verification
The standard EN 15804 serves as the core PCR
Independent verification of the declaration and data according to ISO
14025:2011
internally X externally
Dipl.-Ing. Hans Peters
(Chairman of Institut Bauen und Umwelt e.V.)
Dipl.-Ing. Hans Peters Prof. Dr. Birgit Grahl,
(Managing Director Institut Bauen und Umwelt e.V.) (Independent verifier)
1 Environmental Product Declaration - Stiferite - Stiferite Isocanale Ai8 average thick panel
Product
building equipment and industrial installations - Factory made
Product description/Product definition rigid polyurethane foam (PUR) and polyisocyanurate foam
Stiferite's thermal insulation panels are mainly used in the (PIR) products - Specification and the CE-marking. For the
building/construction sector and in industrial insulation. application and use the respective national provisions apply.
The panels are made of thermo-setting closed cells
polyurethane foam (PU) supplied with various types of flexible Base materials/Ancillary materials
facers on both sides of the panel. The nature/type of facer is a Core material (about 83.9 % of the weight of the declared
function of the type of panel and its application. unit):
Expanded rigid polyurethane foam is distinguished by its
thermal insulation performance, mechanical resistance, Closed-cell Polyiso (PIR) rigid foam made from MDI (50-65 %),
workability, lightness, and durability. polyols (25-35 %), pentane (4-6 %) and additives (4-7 %).
The performance of Stiferite'spanels is determined based on
the European norm EN 14308:2009+A1:2013 - Thermal Facing (about 16.1 % of the weight of the declared unit):
insulation products for building equipment and industrial consisting of aluminium (95-99 %) and lacquer (5-1 %).
installations - Factory made rigid polyurethane foam (PUR) and The PU board for insulation:
polyisocyanurate foam (PIR) products - Specification.
• This product/article/at least one partial article contains
This EPD refers to Stiferite's Isocanale Ai8 average thick panel,
substances listed in the candidate list (date: 17.01.2022)
made of an insulation component in polyurethane foam using
exceeding 0.1 percentage by mass: no
blowing agent Pentane-based, covered on both sides by
embossed aluminium of 80 my thickness. The panel is • This product/article/at least one partial article doesn't
produced in standard dimensions of 1200 x 4000 mm and contain other carcinogenic, mutagenic, reprotoxic
straight finish borders. (CMR) substances in categories 1A or 1B which are not
Upon request and for minimum quantities, the panels may be on the candidate list, exceeding 0.1 percentage by
produced in various dimensions, and the borders may be mass: no
rabbeted along the sides. The surface of the panel may be • Biocide products were added to this construction
evened out with sandpaper in order to allow installation on product or it has been treated with biocide products (this
uneven surfaces. Stiferite Isocanale Ai8 panel is produced by a then concerns a treated product as defined by the (EU)
certified company with systems:ISO 9001, ISO 45001, ISO Ordinance on Biocide Products No.528/2012): no
14001 in its entire line of products. Additional declaration according to quoted law: The product is
compliant with all requirements indicated in chapter 2.5.7
Application
'Isolanti termici ed acustici' of the n.256 D.L. of the 23th June
The Stiferite Isocanale Ai8 panel is suited for the construction of 2022 (CAM EDILIZIA):
pre-insulated heating and ventilation ducts.
• Any blowing agent with Ozone depletion potential >0 is
Technical Data not used in production
In this Life Cycle Assessment, a PU insulation board with the • Any substances of Very High Concern-SVHC in
following properties has been regarded: concentration of more than 0,1 %w are not used in
production (REACH n. 1907/2006). Any specific
Constructional data
authorizations for use are eserved provided for by the
Name Value Unit same Regulation for the substances included in Annex
Gross density 47.6 kg/m3 XIV and specifications restrictions set out in Annex XVII
of the Regulation.
Declared Average Thermal conductivity λi acc.
0.021 W/mK • Catalysts lead-based are not used in production
to EN 14308
• Flame retardants used in production (belonging to the
Water absorption by total immersion acc. to EN Vol.-
<1 Organophosphorus class) are not banned by any
12087 %
national or European regulation
Water absorption by partial immersion acc. to < 0.1 kg/m² • According to the raw materials declarations of suppliers,
EN 1609 the minimum amount of recycled raw materials based
Water vapour diffusion resistance factor μ acc. on the insulation board (PU foam and facers) weight is 3
Endless
to EN 12086 % and the minimum amount of recycled raw materials
w
Euroclass reaction to fire Stiferite Duct acc. to based on the PU insulation foam weight is 4 % in
B-s1,d0 w
EN 13823 compliance with REMADE in Italy type 1 certification
This provides a thermal resistance R = 0.91 m² k/W. (note: this information is not explicitly considered in the
LCA and not included in the EPD tables that only refer
Product according to the CPR based on a to recycling content in the foreground system).
hEN/:14308:2009+A1:2013 For the placing on the market of the
Reference service life
product in the European Union/European Free Trade
The durability of insulation panels is normally at least as long as
Association (EU/EFTA) (with the exception of Switzerland)
the lifetime of the building in which it is used. The experimental
Regulation (EU) No.305/2011 (CPR) applies. The product
data show that the reference life is greater than 50 years.
needs a Declaration of Performance taking into consideration
EN 14308:2009+A1:2013 - Thermal insulation products for
LCA: Calculation rules
The declared unit is 1 m² with a thickness of 20.0 mm, e. g.
Declared Unit 0.020 m³.
Corresponding conversion factors are listed in the table below.
2 Environmental Product Declaration - Stiferite - Stiferite Isocanale Ai8 average thick panel
A2 - Raw material transport
Declared unit
A3 - Production of the insulation board and packaging material
Name Value Unit
A4 - Transport to the construction site
Declared unit 1 m2 C1 - demolition and deconstruction
Gross density 47.6 kg/m3 C2 - Transport to end of life
C3 - End-of-Life: waste management (thermal recovery)
Grammage 1 kg/m2
C4 - End-of-Life: waste management (landfill)
Layer thickness 0.02 m
D - Benefits and loads beyond system boundary
Declared average thermal conductivity λi 0.021 W/mK
Geographic Representativeness
This provides a thermal resistance R = 0.91 m² /W.
Land or region, in which the declared product system is
manufactured, used or handled at the end of the product´s
System boundary lifespan: Italy
Type of the EPD: cradle to gate - with options This life cycle
assessment for the production of the polyurethane insulation
Comparability
board considers the life cycle from the supply of raw materials
Basically, a comparison or an evaluation of EPD data is only
to the manufacturer´s gate (cradle-to-gate with options). It also
possible if all the data sets to be compared were created
includes the transport to the construction site and the end-of-life
according to EN 15804 and the building context, respectively
stage of the used PU thermal insulation board. The life cycle is
the product-specific characteristics of performance, are taken
split into the following individual phases:
into account. The background database used is GaBi 2022
database (v. 2022.1)
A1 - Raw material formulation
LCA: Scenarios and additional technical information
End of life (C1-C4)
Characteristic product properties of biogenic carbon
Name Value Unit
Information on describing the biogenic Carbon Content at
Scenario No 1: Material Incineration 100 %
factory gate
Scenario No 2: Landfill 100 %
Name ValueUnit
kg C1 – Deconstruction and demolition (0.2 MJ/kg as electrical
Biogenic carbon content in product - C consumption assumed)
Biogenic carbon content in accompanying kg
0.068 C2 – Panel is transported from the building site to a treatment
packaging C
plant by truck and an average distance of 100 km is
considered.
Transport to the building site (A4) C3/C4- Disposal scenarios used are divided into 2 sub-
scenarios:
Name ValueUnit
1) Incineration 100 % (C3/1)
Truck with a capacity of 17.3 tons 695 km
2) Landfilling 100 % (C4/2)
Ferry with a capacity of 1200-10000 dwt payload
255 km
capacity
Reuse, recovery and/or recycling potentials (D), relevant
Ship with a capacity of 27500 dwt payload capacity 89,6 km scenario information
tons
D: Benefits and loads beyond system boundary are divided into
Plane with a capacity of 22 ton 0 km 2 sub-scenarios:
Name Value Unit
Type and amount of packaging included in module A3
Scenario No 1: Material Incineration 100 %
Name Value Unit
Scenario No 2: Landfill 100 %
Cardboard 0.15142 kg
EPS stock 0.00578 kg
EPS stock - glue 0.00041 kg
Paper labels 0.00014 kg
PE film 0.01549 kg
PP tape 0.00005 kg
PUR stucks 0 kg
SBR labels 0.00001 kg
TOTAL PACKAGING 0.17372 kg
3 Environmental Product Declaration - Stiferite - Stiferite Isocanale Ai8 average thick panel
LCA: Results
The tables below show the results of the LCA. Basic information on all declared modules provides chapter 4.
There are two scenarios for the end-of-life (C2, C4 and D) analyzed: Scenario 1 considers 100 % incineration, Scenario 2 considers
100 % landfill disposal.
For SM, RSF, NRSF, CRU indicators only the foreground system is considered.
DESCRIPTION OF THE SYSTEM BOUNDARY (X = INCLUDED IN LCA; ND = MODULE OR INDICATOR NOT DECLARED; MNR =
MODULE NOT RELEVANT)
Benefits and
Construction loads beyond
Product stage Use stage End-of-life stage
process stage the system
boundaries
la ire ta m w a Ry lp p u s tro p s n a rT g n iru tc a fu n a M e h t m o rf tro p s n a rTe tis e h t o t e ta g y lb m e s s A e s U e c n a n e tn ia M ria p e R tn e m e c a lp e R tn e m h s ib ru fe R y g re n e la n o ita re p Oe s u re ta w la n o ita re p Oe s u n o itc u rts n o c -e Dn o itilo m e d tro p s n a rT g n is s e c o rp e ts a W la s o p s iD -e s u e R-y re v o c e R-g n ilc y c e Rla itn e to p
A1 A2 A3 A4 A5 B1 B2 B3 B4 B5 B6 B7 C1 C2 C3 C4 D
X X X X MND MND MND MNR MNR MNR MND MND X X X X X
RESULTS OF THE LCA - ENVIRONMENTAL IMPACT according to EN 15804+A2: 1 m2 Isocanale Ai8
Parameter Unit A1-A3 A4 C1 C2 C3/1 C3/2 C4/1 C4/2 D/1 D/2
GWP-total kg CO 2 eq 3.76E+00 7.39E-02 2.17E-02 5.74E-03 1.77E+00 0 0 1.43E-02 -8.34E-01 0
GWP-fossil kg CO 2 eq 4.06E+00 7.32E-02 2.16E-02 5.68E-03 1.77E+00 0 0 1.42E-02 -8.33E-01 0
GWP-
biogenic kg CO 2 eq -3.08E-01 2.13E-04 1.28E-05 1.84E-05 1.44E-04 0 0 4.41E-05 -7.48E-04 0
GWP-luluc kg CO 2 eq 1.94E-03 4.06E-04 1.4E-06 3.82E-05 1.07E-05 0 0 2.6E-05 -4.51E-05 0
ODP kg CFC11 eq 5.98E-12 6.72E-15 2.14E-13 5.57E-16 2.17E-13 0 0 3.33E-14 -6.13E-12 0
AP mol H+ eq 1.07E-02 4.84E-04 3.18E-05 1.89E-05 1.07E-03 0 0 1E-04 -1.03E-03 0
EP-
kg P eq 1.03E-05 2.18E-07 9.71E-09 2.02E-08 8.21E-08 0 0 5.15E-08 -2.91E-07 0
freshwater
EP-marine kg N eq 2.22E-03 2.23E-04 8.69E-06 8.66E-06 5.14E-04 0 0 2.56E-05 -3E-04 0
EP-terrestrial mol N eq 2.32E-02 2.47E-03 9.28E-05 9.7E-05 5.91E-03 0 0 2.81E-04 -3.23E-03 0
kg NMVOC
POCP 9.66E-03 5.29E-04 2.45E-05 1.7E-05 1.32E-03 0 0 7.78E-05 -8.55E-04 0
eq
ADPE kg Sb eq 8.5E-07 6.61E-09 2.57E-09 5.71E-10 5.33E-09 0 0 1.45E-09 -8.37E-08 0
ADPF MJ 7.9E+01 9.66E-01 4.59E-01 7.44E-02 7.33E-01 0 0 1.86E-01 -1.66E+01 0
m3 world eq
WDP 7.21E-01 6.99E-04 1.62E-03 6.34E-05 1.91E-01 0 0 1.54E-03 -4.68E-02 0
deprived
GWP = Global warming potential; ODP = Depletion potential of the stratospheric ozone layer; AP = Acidification potential of land and water; EP =
Eutrophication potential; POCP = Formation potential of tropospheric ozone photochemical oxidants; ADPE = Abiotic depletion potential for non-fossil
resources; ADPF = Abiotic depletion potential for fossil resources; WDP = Water (user) deprivation potential)
RESULTS OF THE LCA - INDICATORS TO DESCRIBE RESOURCE USE according to EN 15804+A2: 1 m2 Isocanale Ai8
Parameter Unit A1-A3 A4 C1 C2 C3/1 C3/2 C4/1 C4/2 D/1 D/2
PERE MJ 9.15E+00 5.55E-02 6.63E-02 5.16E-03 1.17E-01 0 0 2.78E-02 -1.91E+00 0
PERM MJ 2.67E+00 ND ND ND ND 0 0 ND ND 0
PERT MJ 1.18E+01 5.55E-02 6.63E-02 5.16E-03 1.17E-01 0 0 2.78E-02 -1.91E+00 0
PENRE MJ 5.66E+01 9.7E-01 4.59E-01 7.47E-02 2.22E+01 0 0 2.16E+01 -1.66E+01 0
PENRM MJ 2.25E+01 ND ND ND -2.14E+01 0 0 -2.14E+01 ND 0
PENRT MJ 7.91E+01 9.7E-01 4.59E-01 7.47E-02 7.34E-01 0 0 1.87E-01 -1.66E+01 0
SM kg 2.77E-01 ND ND ND ND 0 0 ND ND 0
RSF MJ ND ND ND ND ND 0 0 ND ND 0
NRSF MJ ND ND ND ND ND 0 0 ND ND 0
FW m3 3.63E-02 6.44E-05 1E-04 5.96E-06 4.5E-03 0 0 4.68E-05 -2.9E-03 0
PERE = Use of renewable primary energy excluding renewable primary energy resources used as raw materials; PERM = Use of renewable primary
energy resources used as raw materials; PERT = Total use of renewable primary energy resources; PENRE = Use of non-renewable primary energy
excluding non-renewable primary energy resources used as raw materials; PENRM = Use of non-renewable primary energy resources used as raw
materials; PENRT = Total use of non-renewable primary energy resources; SM = Use of secondary material; RSF = Use of renewable secondary fuels;
NRSF = Use of non-renewable secondary fuels; FW = Use of net fresh water
RESULTS OF THE LCA – WASTE CATEGORIES AND OUTPUT FLOWS according to EN 15804+A2:
1 m2 Isocanale Ai8
Parameter Unit A1-A3 A4 C1 C2 C3/1 C3/2 C4/1 C4/2 D/1 D/2
HWD kg 1.7E-08 4.8E-12 3.28E-11 3.95E-13 8.99E-11 0 0 9.8E-12 -1.56E-09 0
NHWD kg 4.68E-01 1.46E-04 9.75E-05 1.22E-05 7.73E-02 0 0 9.45E-01 -3.68E-03 0
RWD kg 1.87E-03 1.67E-06 7.63E-05 1.39E-07 4.26E-05 0 0 2.08E-06 -2.18E-03 0
CRU kg ND ND ND ND ND 0 0 ND ND 0
4 Environmental Product Declaration - Stiferite - Stiferite Isocanale Ai8 average thick panel
MFR kg ND ND ND ND ND 0 0 ND ND 0
MER kg ND ND ND ND ND 0 0 ND ND 0
EEE MJ ND ND ND ND 5.41E+00 0 0 ND ND 0
EET MJ ND ND ND ND 3.04E+00 0 0 ND ND 0
HWD = Hazardous waste disposed; NHWD = Non-hazardous waste disposed; RWD = Radioactive waste disposed; CRU = Components for re-use;
MFR = Materials for recycling; MER = Materials for energy recovery; EEE = Exported electrical energy; EET = Exported thermal energy
RESULTS OF THE LCA – additional impact categories according to EN 15804+A2-optional:
1 m2 Isocanale Ai8
Parameter Unit A1-A3 A4 C1 C2 C3/1 C3/2 C4/1 C4/2 D/1 D/2
Disease
PM 1.04E-07 5.79E-09 2.84E-10 1.08E-10 3.61E-09 0 0 1.23E-09 -9.12E-09 0
incidence
IR kBq U235 eq 3.15E-01 2.51E-04 1.12E-02 2.09E-05 6.52E-03 0 0 2.33E-04 -3.2E-01 0
ETP-fw CTUe 3.09E+01 6.83E-01 1.41E-01 5.27E-02 2.57E-01 0 0 3.36E+00 -4.05E+00 0
HTP-c CTUh 2.48E-09 1.38E-11 2.59E-12 1.09E-12 1.52E-11 0 0 1.58E-11 -1E-10 0
HTP-nc CTUh 1.73E-07 8.23E-10 1.32E-10 6.66E-11 6.7E-10 0 0 1.75E-09 -4.85E-09 0
SQP SQP 9.5E+00 3.35E-01 4.21E-02 3.15E-02 1.33E-01 0 0 3.85E-02 -1.21E+00 0
PM = Potential incidence of disease due to PM emissions; IR = Potential Human exposure efficiency relative to U235; ETP-fw = Potential comparative
Toxic Unit for ecosystems; HTP-c = Potential comparative Toxic Unit for humans (cancerogenic); HTP-nc = Potential comparative Toxic Unit for humans
(not cancerogenic); SQP = Potential soil quality index
Disclaimer 1 – for the indicator “Potential Human exposure efficiency relative to U235”. This impact category deals mainly with the
eventual impact of low-dose ionizing radiation on human health of the nuclear fuel cycle. It does not consider effects due to possible
nuclear accidents, occupational exposure or radioactive waste disposal in underground facilities. Potential ionizing radiation from the
soil, radon and from some construction materials is also not measured by this indicator.
Disclaimer 2 – for the indicators “abiotic depletion potential for non-fossil resources”, “abiotic depletion potential for fossil resources”,
“water (user) deprivation potential, deprivation-weighted water consumption”, “potential comparative toxic unit for ecosystems”,
“potential comparative toxic unit for humans – cancerogenic”, “Potential comparative toxic unit for humans - not cancerogenic”,
“potential soil quality index”. The results of this environmental impact indicator shall be used with care as the uncertainties on these
results are high as there is limited experience with the indicator.
References
Standards CPR ISO 9001:2015 Quality management
Regulation (EU) No.305/2011 laying down harmonised
conditions for the marketing of construction products and ISO 14001
repealing Council Directive 89/106/EEC ISO 14001: 2015 Environmental management systems
EN 1609 ISO 14025
EN 1609: Thermal insulating products for building applications. EN ISO 14025:2011 Environmental labels and declarations —
Determination of short term water absorption by partial Type III environmental declarations - Principles and procedures.
immersion.
ISO 45001
EN 13823 ISO 45001: 2018 Occupational health and safety management
EN 13823:2020 Reaction to fire tests for building products - systems
Building products excluding floorings exposed to the thermal
attack by a single burning item GaBi 2022
GaBi 10 and DB 2022.1: Documentation of GaBi 10: Software-
EN 12086 System and Database for Life Cycle Engineering. Copyright,
EN 12086: 2013 Thermal insulating products for building TM. Stuttgart, Leinfelden-Echterdingen, 1992-2022
applications. Determination of water vapour transmission http://www.gabi-software.com
properties.
IBU 2021
EN 12087 Institut Bauen und Umwelt e.V.: General Instructions for the
EN 12087:2013 Thermal insulating products for building EPD programme of Institut Bauen und Umwelt e.V., Version
applications. Determination of long term water absorption by 2.0, Berlin: Institut Bauen und Umwelt e.V., 2021 www.ibu-
immersion. epd.com
EN 14308 IBU PCR Part A
EN 14308:2009+A1:2013 - Thermal insulation products for Product Category Rules for Building-Related Products and
building equipment and industrial installations - Factory made Services. Part A: Calculation Rules for the Life Cycle
rigid polyurethane foam (PUR) and polyisocyanurate foam Assessment and Requirements on the Project Report according
(PIR) products - Specification to EN 15804+A2:2019; V1.2, 11/2021
EN 15804 IBU PCR Part B
EN 15804:2012+A2:2019+AC:2021 Sustainability of PCR Guidance-Texts for Building-Related Products and
construction works — Environmental Product Declarations — Services; Part B: Requirements on the EPD for Insulating
Core rules for the product category of construction products. materials made of foam plastics; Institute Construction and
Environment e.V. (IBU). Version 01.2019 https://epd-online.com
ISO 9001
5 Environmental Product Declaration - Stiferite - Stiferite Isocanale Ai8 average thick panel
PANGPP 2022 Ordinance on Biocide Products
Piano d' Azione Nazionale sul Green Public Procurement Regulation (eu) n. 528/2012 of the European Parliament and of
(PANGPP) – Decreto Ministeriale n. 256 del 23-06-2022 the Council of 22 May 2012 concerning the making available on
Gazzetta Ufficiale della Repubblica Italiana, Serie Generale the market and use of biocidal products Text with EEA
n.183 del 06-08-2022 https://www.mite.gov.it/notizie/novita-sui- relevance
criteri-minini-ambientali-cam
REMADE IN ITALY
REACH Certificate No.1245/001 for Stiferite Rev. n. 0 18 November
REACH Registration, Evaluation, Authorization and Restriction 2021
of Chemical, 2007
STIFERITE LCA tool background report v 2.3 (03-06-2022)
6 Environmental Product Declaration - Stiferite - Stiferite Isocanale Ai8 average thick panel
Publisher
Institut Bauen und Umwelt e.V. +49 (0)30 3087748- 0
Hegelplatz 1 info@ibu-epd.com
10117 Berlin www.ibu-epd.com
Germany
Programme holder
Institut Bauen und Umwelt e.V. +49 (0)30 3087748- 0
Hegelplatz 1 info@ibu-epd.com
10117 Berlin www.ibu-epd.com
Germany
Author of the Life Cycle Assessment
Sphera Solutions GmbH +49 711 341817-0
Hauptstraße 111- 113 info@sphera.com
70771 Leinfelden-Echterdingen www.sphera.com
Germany
Owner of the Declaration
Stiferite +39 049 8997911
Viale Navigazione Interna 54 info@stiferite.com
35129 Padova www.stiferite.com
Italy
7 Environmental Product Declaration - Stiferite - Stiferite Isocanale Ai8 average thick panel
