ENVIRONMENTAL
as per ISO 14025 and EN 15804+A2
Owner of the Declaration Interface®
Programme holder Institut Bauen und Umwelt e.V. (IBU)
Publisher Institut Bauen und Umwelt e.V. (IBU)
Declaration number EPD-INT-20220230-CBB1-EN
Issue date 17.02.2023
Valid to 16.02.2028
Superfloor II
Modular needled carpet tiles
with a CQuest bio backing
Interface®
www.ibu-epd.com | https://epd-online.com
Umwelt Produktdeklaration Name des Herstellers – Name des Produkts
General Information
Interface® Superfloor II Modular needled carpet
tiles
with a CQuest bio backing
Programme holder Owner of the declaration
IBU – Institut Bauen und Umwelt e.V. Interface Europe Manufacturing BV
Hegelplatz 1 Industrielaan 15
10117 Berlin 3925 ZG Scherpenzeel
Germany The Netherlands
Declaration number Declared product / declared unit
EPD-INT-20220230-CBB1-EN 1 m² needled modular carpet tiles with polypropylene
felt covered heavy backing and a pile material of
polyamide 6, polypropylene and polyester with 87%
recycled content
This declaration is based on the product Scope:
category rules: The manufacturer declaration applies to needled
Floor coverings, 02/2018 carpet tiles with a polypropylene felt covered heavy
(PCR checked and approved by the SVR) backing, a pile material of PA 6, PP and PET with a
maximum total pile weight of 521 g/m2. The products
are needled in Genemuiden, the Netherlands. The
Issue date
carpets are back coated in Scherpenzeel.
17.02.2023
The declaration is only valid in conjunction with a valid
GUT-PRODIS license of the product.
Valid to
16.02.2028
The owner of the declaration shall be liable for the
underlying information and evidence; the IBU shall not
be liable with respect to manufacturer information, life
cycle assessment data and evidences.
The EPD was created according to the specifications
of EN 15804+A2. In the following, the standard will be
simplified as EN 15804.
Verification
The standard EN 15804 serves as the core PCR
Independent verification of the declaration and data
according to ISO 14025:2011
Dipl. Ing. Hans Peters internally x externally
(chairman of Institut Bauen und Umwelt e.V.)
Dr. Alexander Röder Prof. Dr. Birgit Grahl
(Managing Director Institut Bauen und Umwelt e.V.)) (Independent verifier)
Product
Product description/Product definition consideration EN 14041:2018-05, Resilient, textile and
The declaration applies to needled carpet tiles having laminate floor coverings - Essential characteristics, and
a surface pile of mainly solution-dyed PA 6, PP and the CE-marking. The DoP of the product can be found
PET with a total pile weight of 521 g/m2. The backing on the manufacturer's technical information section.
of the carpet consists of a CQuest Bio heavy backing For the application and use of the product the
covered by a polypropylene felt. The total recycled respective national provisions apply.
content of the carpet is 62%.
CQuest Bio backing system: Backing compound based Application
on renewable wood resin, containing a recycled filler The use class of the specific product as defined in
and glass-fleece reinforcement. EN 1307 can be found in the Product Information
For the placing on the market of the specific product in System (PRODIS) using the PRODIS registration
the European Union/European Free Trade Association number of the product.
(EU/EFTA) (with the exception of Switzerland)
Regulation (EU) No. 305/2011 Construction Product Technical Data
Regulation (CPR) applies. The product needs a
Declaration of Performance (DoP) taking into
Constructional data according to EN 1307
2 Environmental Product Declaration Interface – Superfloor II, Needled tiles with a total pile weight of 521 g/m2 and a
CQuest Bio backing
Name Value Unit Glass fiber 0.5 %
Modular carpet tiles, 50 cm x The specific product covered by the EPD contains
Product Form -
50 cm substances listed in the ECHA candidate list
Type of (08.07.2021) exceeding 0.1 percentage by mass: no
Needled carpet -
manufacture This product contains other CMR substances in
Polyamide 6, polypropylene categories 1A or 1B which are not on the candidate list
Yarn type and polyester from 87% - exceeding 0.1 percentage by mass: no
recycled material Biocide products were added to this construction
Total carpet weight 4045 g/m2 product or it has been treated with biocide products
CQB backing with a PP felt (this then concerns a treated product as defined by the
Secondary backing -
bottom (EU) Ordinance on Biocide Products No. 528/2012): no
Aluminium hydroxide is used as fire retardant.
Performance data of the product in accordance with Reference service life
the declaration of performance with respect to its The service life of textile floor coverings strongly
essential characteristics according to EN 14041: 2018- depends on the correct installation taking into account
05, Resilient, textile and laminate floor coverings - the declared use classification and the adherence to
Essential characteristics. cleaning and maintenance instructions.
Additional product properties in accordance with EN A calculation of the reference service life according to
1307 can be found on the Product Information System ISO 15686 is not possible.
PRODIS using the PRODIS registration number of the Alternatively, a reference service life of 15 years can
product (www.pro-dis.info) or on the manufacturer's be assumed, during which the functional and visual
technical information section. quality is guaranteed. This is in accordance with the
product the warranty of the manufacturer. The
Base materials/Ancillary materials technical service life can be significantly longer.
Name Value Unit
Polyester 12.5 %
Polyamide 6 9.0 %
Polypropylene 2.5 %
Ethylene vinyl acetate (EVA) 5.9 %
Wood resin 8.1 %
Additives 2.1 %
Limestone 59.4 %
LCA: Calculation rules
Declared Unit of production waste are aggregated.
Biogenic carbon that is stored in renewable material
(wood resin, renewable additives,packaging paper) is
Name Value Unit taken into account as well as the associated carbon
Declared unit 1 m2 dioxide uptake from the air from which this biogenic
Grammage 4.045 kg/m2 carbon comes.
Total thickness 6.9 mm
Gross density 586 kg/m3 A4 Transport:
The declared unit refers to 1 m2 produced textile floor Transport of the packed textile floor covering
covering. The output of module A5 'Assembly' is 1 m2 from factory gate to the place of installation.
installed textile floor covering.
A5 Installation:
Installation of the textile floor covering, processing of
installation waste and packaging waste up to the
System boundary landfill disposal of residual waste (except radioactive
waste), the production of the amount of carpet that
Type of EPD: Cradle-to-gate with options occurs as installation waste including its transport to
System boundaries of modules A, B, C, D: the place of installation.
Modules C3, C4 and D are indicated separately for Generated electricity and steam due to the incineration
three end-of-life scenarios: of waste are listed in the result table as exported
1 - landfill disposal energy.
2 - municipal waste incineration Biogenic carbon that is stored in renewable materials
3 - recovery in a cement plant in installation waste and packaging paper is released
as carbon dioxide emissions into the air at the end of
A1-A3 Production: life in module A5.
Energy supply and production of the basic material, Preparation of the floor and auxiliary materials
processing of secondary material, auxiliary material, (adhesives, fixing agents, PET connectors) are beyond
transport of the material to the manufacturing site, the system boundaries and not taken into account.
emissions, waste water treatment, packaging material
and waste processing up to the landfill disposal of B1 Use:
residual waste (except radioactive waste). Benefits for Indoor emissions during the use stage. After the first
generated electricity and steam due to the incineration year, no product-related Volatile Organic Compound
3 Environmental Product Declaration Interface – Superfloor II, Needled tiles with a total pile weight of 521 g/m2 and a
CQuest Bio backing
(VOC) emissions are relevant due to known VOC transport to the cement plant, emissions from the
decay curves of the product. incineration.
B2 Maintenance: C4 Disposal
Cleaning of the textile floor covering for a period of 1 C4-1: Impact from landfill disposal,
year: C4-2: The carpet waste leaves the system in module
Vacuum cleaning – electricity supply C3-2,
Wet cleaning – electricity, water consumption, C4-3: The pre-processed carpet waste leaves the
production of the cleaning agent, waste water system in module C3-3.
treatment
The declared values in this module have to be D Recycling potential:
multiplied by the assumed service life of the floor Calculated benefits result from materials exclusive
covering in the building in question. secondary materials (net materials).
D-A5: Benefits for generated energy due
B3 - B5: to incineration of packaging and installation waste
The modules are not relevant within the assumed (incineration plant with R1 > 0.6),
reference service life of 15 years. D-1: Assuming that the chemically bound renewable
materials in a landfill gas do not release landfill gas
B6 - B7: within 100 years, no benefits due to landfill dosposal of
No energy and water input are required for the carpet waste at the end-of-life are taken into account,
operation of the carpet in the use stage. The modules D-2: Benefits for generated energy due to incineration
do not cause any environmental impact. of carpet waste at the end-of-life (incineration plant
with R1 > 0.6),
C1 De-construction: D-3: Benefits for saved fossil energy and saved
The floor covering is de-constructed manually and no inorganic material due to recovery of the carpet in a
additional environmental impact is caused. cement plant.
C2 Transport: Comparability
Transport of the carpet waste to a landfill, to the Basically, a comparison or an evaluation of EPD data
municipal waste incineration plant (MWI) or to the is only possible if all the data sets to be compared
waste collection facility for recycling. were created according to EN 15804 and the building
context, respectively the product-specific
C3 Waste processing: characteristics of performance, are taken into account.
C3-1: Landfill disposal needs no waste processing.
C3-2: Impact from waste incineration (plant with R1 > Background data are taken from the GaBi database,
0.6), generated electricity and steam are listed in the 2022-1. Remaining data gaps are covered by the
result table as exported energy. ecoinvent 3.7 database, 2020.
C3-3: Collection of the carpet waste for recovery in the
cement industry, waste processing (granulating),
LCA: Scenarios and additional technical information
Characteristic product properties to be recycled.
Information on biogenic Carbon Preparation of the floor and auxiliaries (adhesives,
fixing agents, PET connectors etc.) are not taken into
account.
Name Value Unit
Biogenic carbon content in Maintenance (B2)
0.3 kg C
product at factory gate The values for cleaning refer to 1 m2 floor covering per
Biogenic carbon content in year.
accompanying packaging at 0.05 kg C Depending on the application based on ISO 10874, the
factory gate technical service life recommended by the
1 kg biogenic Carbon is equivalent to 44/12 kg of CO manufacturer and the anticipated strain on the floor by
2
customers, the case-specific useful life can be
established. Based on this useful life the effects of
module B2 need to be calculated in order to obtain the
Transport to the construction site (A4) overall environmental impacts.
Name Value Unit
Litres of fuel (truck, EURO 0-6
0.0095 l/100km
mix) Name Value Unit
Transport distance 700 km Number
Maintenance cycle (vacuum cleaning) 208
Capacity utilisation (including /year
55 %
empty runs) Number
Maintenance cycle (wet cleaning) 1,5
/year
Installation in the building (A5) Water consumption (wet cleaning) 0.004 m3
Name Value Unit Cleaning agent (wet cleaning) 0.09 kg
Material loss 0.121 kg Electricity consumption 0.314 kWh
Polyethylene packaging waste and installation waste For further information on cleaning and maintenance
are considered to be incinerated in a municipal waste see www.interface.com
incineration plant. Cardboard packaging waste is going
4 Environmental Product Declaration Interface – Superfloor II, Needled tiles with a total pile weight of 521 g/m2 and a
CQuest Bio backing
Service life
Name Value Unit
Life Span (according to
15 a
manufacturer's warranty)
Declared product
Corresponds to the
properties (at the gate) -
specifications of EN 1307
and finishes
An assumed quality of
work, when installed in Conforms to the
accordance with the manufacturer's -
manufacturer’s instructions
instructions
Usage conditions, e.g. Use in areas defined by
frequency of use, the use class according -
mechanical exposure to EN 1307
Maintenance e.g.
required frequency, type According to the
and quality and manufacturers -
replacement of instructions
components
End of Life (C1-C4)
Three different end-of-life scenarios are declared and
the results are indicated separately in module C.
Each scenario is calculated as a 100% scenario.
Scenario 1: 100 % landfill disposal
Scenario 2: 100 % municipal waste incineration (MWI)
with R1 > 0.6
Scenario 3: 100 % recovery in the cement industry
If combinations of these scenarios have to be
calculated this should be done according to the
following scheme:
EOL-impact = x % impact (Scenario 1)
+ y % impact (Scenario 2)
+ z % impact (Scenario 3)
with x % + y % + z % = 100 %
Name Value Unit
Collected as mixed construction
4.045 kg
waste (scenario 1 and 2)
Collected separately (scenario 3) 4.045 kg
Landfilling (scenario 1) 4.045 kg
Energy recovery (scenario 2) 4.045 kg
Energy recovery (scenario 3) 1.621 kg
Recycling (scenario 3) 2.424 kg
Reuse, recovery and/or recycling potentials (D),
relevant scenario information
Recovery or recycling potentials due to the three end-
of-life scenarios (module C) are indicated separately.
Recycling in the cement industry (scenario 3)
The organic material of the carpet is used as an
alternative fuel in a cement kiln. It mainly substitutes
for lignite (68.8%), hard coal (23.6%) and petrol coke
(7.6%). The inorganic material is substantially
integrated into the cement clinker and substitutes for
original material input. VDZ e.V.
5 Environmental Product Declaration Interface – Superfloor II, Needled tiles with a total pile weight of 521 g/m2 and a
CQuest Bio backing
LCA: Results
The LCA results refer to the declared product with a total pile weight of 521 g/m2. The declared result figures in
module B2 have to be multiplied by the assumed service life (in years) of the floor covering in the building under
consideration. Information on non-relevant modules: Modules B3 - B7 are not relevant during the service life of
the carpet. Modules C1, C3/1, C4/2 and C4/3 cause no additional impact (see chapter "LCA: Calculation rules" in
this document). All these modules are declared and marked as 'modules not relevant/declared'. Module C2
represents the transport for scenarios 1, 2 and 3. Column D represents benefits from module A5 assembly.
DESCRIPTION OF THE SYSTEM BOUNDARY (X = INCLUDED IN LCA; ND = MODULE OR INDICATOR NOT
DECLARED; MNR = MODULE NOT RELEVANT)
BENEFITS AND
CONSTRUCTI LOADS
PRODUCT STAGE ON PROCESS USE STAGE END OF LIFE STAGE BEYOND THE
STAGE SYSTEM
BOUNDARIES
6 Environmental Product Declaration Interface – Superfloor II, Needled tiles with a total pile weight of 521 g/m2 and a
CQuest Bio backing
lairetam
waR
ylppus tropsnarT
gnirutcafunaM
eht
morf
tropsnarT
etis
eht
ot
etag
ylbmessA esU
ecnanetniaM
riapeR
tnemecalpeR tnemhsibrufeR
ygrene
lanoitarepO esu
retaw
lanoitarepO esu
noitcurtsnoc-eD
noitilomed tropsnarT
gnissecorp
etsaW
lasopsiD -esueR -yrevoceR -gnilcyceR laitnetop
A1 A2 A3 A4 A5 B1 B2 B3 B4 B5 B6 B7 C1 C2 C3 C4 D
X X X X X X X MNR MNR MNR ND ND X X X X X
RESULTS OF THE LCA - ENVIRONMENTAL IMPACT according to EN 15804+A2: 1 m² floor covering
Core Indicator Unit A1-A3 A4 A5 B1 B2 C1 C2 C3/2 C3/3 C4/1 D D/1 D/2 D/3
-
GWP-total [kg CO2-Eq.] 1.31E+12.48E-1 6.20E-10.00E+04.16E-10.00E+01.37E-24.31E+04.36E+01.39E+0-4.50E-20.00E+0 1.04E+0-2.52E-1
-
GWP-fossil [kg CO2-Eq.] 1.43E+12.44E-1 5.94E-10.00E+02.15E-10.00E+01.35E-23.20E+03.25E+02.84E-1-4.48E-20.00E+0 1.04E+0-2.52E-1
-
GWP-biogenic [kg CO2-Eq.] 1.15E+03.15E-3 2.59E-20.00E+04.16E-30.00E+01.74E-41.11E+01.11E+01.11E+0-2.29E-40.00E+0-5.31E-3-2.85E-4
GWP-luluc [kg CO2-Eq.] 1.11E-2 1.38E-3 3.85E-40.00E+01.96E-10.00E+07.63E-5 2.46E-4 4.42E-4 1.40E-4-4.92E-60.00E+0-1.14E-4-1.05E-4
1.48E- 4.10E- 8.20E- 3.03E- 6.08E- 3.85E- -3.03E- -7.01E- -4.67E-
ODP [kg CFC11-Eq.] 1.37E-8 0.00E+03.42E-80.00E+0 0.00E+0
14 10 16 13 13 13 13 12 13
AP [mol H+-Eq.] 2.49E-2 1.47E-3 8.73E-40.00E+08.32E-40.00E+08.15E-5 2.52E-3 2.77E-3 8.50E-4-5.89E-50.00E+0-1.36E-3-7.30E-4
EP-freshwater [kg P-Eq.] 1.25E-4 7.38E-7 3.78E-60.00E+05.19E-60.00E+04.09E-8 8.41E-7 1.00E-6 5.35E-5-6.16E-80.00E+0-1.43E-6-2.49E-7
EP-marine [kg N-Eq.] 7.40E-3 7.23E-4 2.81E-40.00E+01.97E-40.00E+04.00E-5 1.16E-3 1.27E-3 1.88E-4-1.60E-50.00E+0-3.70E-4-2.48E-4
EP-terrestrial [mol N-Eq.] 7.43E-2 8.00E-3 2.89E-30.00E+02.83E-30.00E+04.43E-4 1.31E-2 1.43E-2 2.06E-3-1.71E-40.00E+0-3.97E-3-2.71E-3
POCP [kg NMVOC-Eq.]2.45E-2 1.37E-3 8.71E-4 4.18E-4 9.83E-40.00E+07.57E-5 3.00E-3 3.21E-3 6.05E-4-4.47E-50.00E+0-1.04E-3-7.69E-4
ADPE [kg Sb-Eq.] 3.85E-6 2.07E-8 1.17E-70.00E+02.30E-70.00E+01.15E-9 2.29E-8 3.15E-8 1.99E-8-6.75E-90.00E+0-1.57E-7-2.25E-8
- -
ADPF [MJ] 3.87E+23.31E+01.18E+10.00E+05.90E+00.00E+01.83E-12.57E+03.40E+04.07E+0-7.61E-10.00E+0
1.77E+14.09E+1
[m³ world-Eq
WDP 1.49E+12.21E-3 4.68E-10.00E+09.99E-20.00E+01.22E-4 6.05E-1 6.10E-1-3.04E-3-4.72E-30.00E+0-1.09E-1-4.09E-2
deprived]
GWP = Global warming potential; ODP = Depletion potential of the stratospheric ozone layer; AP = Acidification potential of land and water; EP =
Caption Eutrophication potential; POCP = Formation potential of tropospheric ozone photochemical oxidants; ADPE = Abiotic depletion potential for non-
fossil resources; ADPF = Abiotic depletion potential for fossil resources; WDP = Water (user) deprivation potential
RESULTS OF THE LCA - INDICATORS TO DESCRIBE RESOURCE USE according to EN 15804+A2: 1 m²
floor covering
Indicator Unit A1-A3 A4 A5 B1 B2 C1 C2 C3/2 C3/3 C4/1 D D/1 D/2 D/3
PERE [MJ] 5.34E+1 1.88E-1 2.36E+0 0.00E+0 3.69E+0 0.00E+0 1.04E-2 1.62E+1 1.64E+1 3.34E-1 -2.09E-1 0.00E+0 -4.84E+0-2.80E-1
PERM [MJ] 1.59E+1 0.00E+0 -2.60E-1 0.00E+0 0.00E+0 0.00E+0 0.00E+0 -1.57E+1-1.57E+1 0.00E+0 0.00E+0 0.00E+0 0.00E+0 0.00E+0
PERT [MJ] 6.94E+1 1.88E-1 2.10E+0 0.00E+0 3.69E+0 0.00E+0 1.04E-2 4.66E-1 7.01E-1 3.34E-1 -2.09E-1 0.00E+0 -4.84E+0-2.80E-1
PENRE [MJ] 3.56E+2 3.31E+0 1.22E+1 0.00E+0 5.90E+0 0.00E+0 1.83E-1 3.32E+1 3.40E+1 4.07E+0 -7.61E-1 0.00E+0 -1.77E+1-4.09E+1
PENRM [MJ] 3.10E+1 0.00E+0 -3.96E-1 0.00E+0 0.00E+0 0.00E+0 0.00E+0 -3.06E+1-3.06E+1 0.00E+0 0.00E+0 0.00E+0 0.00E+0 0.00E+0
PENRT [MJ] 3.87E+2 3.31E+0 1.18E+1 0.00E+0 5.90E+0 0.00E+0 1.83E-1 2.57E+0 3.40E+0 4.07E+0 -7.61E-1 0.00E+0 -1.77E+1-4.09E+1
SM [kg] 2.57E+0 0.00E+0 7.72E-2 0.00E+0 0.00E+0 0.00E+0 0.00E+0 0.00E+0 0.00E+0 0.00E+0 0.00E+0 0.00E+0 0.00E+0 2.00E-2
RSF [MJ] 0.00E+0 0.00E+0 0.00E+0 0.00E+0 0.00E+0 0.00E+0 0.00E+0 0.00E+0 0.00E+0 0.00E+0 0.00E+0 0.00E+0 0.00E+0 0.00E+0
NRSF [MJ] 0.00E+0 0.00E+0 0.00E+0 0.00E+0 0.00E+0 0.00E+0 0.00E+0 0.00E+0 0.00E+0 0.00E+0 0.00E+0 0.00E+0 0.00E+0 0.00E+0
FW [m³] 4.28E-1 2.12E-4 1.33E-2 0.00E+0 3.34E-3 0.00E+0 1.18E-5 1.43E-2 1.45E-2 4.76E-5 -2.00E-4 0.00E+0 -4.63E-3 -3.55E-3
PERE = Use of renewable primary energy excluding renewable primary energy resources used as raw materials; PERM = Use of
renewable primary energy resources used as raw materials; PERT = Total use of renewable primary energy resources; PENRE = Use of
non-renewable primary energy excluding non-renewable primary energy resources used as raw materials; PENRM = Use of non-
Caption
renewable primary energy resources used as raw materials; PENRT = Total use of non-renewable primary energy resources; SM = Use
of secondary material; RSF = Use of renewable secondary fuels; NRSF = Use of non-renewable secondary fuels; FW = Use of net fresh
water
RESULTS OF THE LCA – WASTE CATEGORIES AND OUTPUT FLOWS according to EN 15804+A2:
1 m² floor covering
Indicator Unit A1-A3 A4 A5 B1 B2 C1 C2 C3/2 C3/3 C4/1 D D/1 D/2 D/3
HWD [kg] 2.62E-7 1.59E-11 7.87E-9 0.00E+0 4.19E-5 0.00E+0 8.78E-133.67E-104.02E-106.27E-10-1.03E-100.00E+0 -2.39E-9-7.02E-11
NHWD [kg] 2.02E-1 4.75E-4 4.27E-2 0.00E+0 7.30E-3 0.00E+0 2.63E-5 1.21E+0 1.21E+0 4.03E+0 -3.85E-4 0.00E+0 -8.92E-3 -7.89E-4
RWD [kg] 6.66E-3 4.08E-6 2.03E-4 0.00E+0 3.76E-4 0.00E+0 2.26E-7 1.03E-4 1.64E-4 5.00E-5 -5.99E-5 0.00E+0 -1.39E-3 -5.59E-5
CRU [kg] 0.00E+0 0.00E+0 0.00E+0 0.00E+0 0.00E+0 0.00E+0 0.00E+0 0.00E+0 0.00E+0 0.00E+0 0.00E+0 0.00E+0 0.00E+0 0.00E+0
MFR [kg] 0.00E+0 0.00E+0 1.21E-1 0.00E+0 0.00E+0 0.00E+0 0.00E+0 0.00E+0 1.37E+0 0.00E+0 0.00E+0 0.00E+0 0.00E+0 0.00E+0
MER [kg] 0.00E+0 0.00E+0 0.00E+0 0.00E+0 0.00E+0 0.00E+0 0.00E+0 0.00E+0 0.00E+0 0.00E+0 0.00E+0 0.00E+0 0.00E+0 0.00E+0
EEE [MJ] 0.00E+0 0.00E+0 1.87E-1 0.00E+0 0.00E+0 0.00E+0 0.00E+0 4.17E+0 0.00E+0 0.00E+0 0.00E+0 0.00E+0 0.00E+0 0.00E+0
EET [MJ] 0.00E+0 0.00E+0 3.49E-1 0.00E+0 0.00E+0 0.00E+0 0.00E+0 8.00E+0 4.84E+1 0.00E+0 0.00E+0 0.00E+0 0.00E+0 0.00E+0
HWD = Hazardous waste disposed; NHWD = Non-hazardous waste disposed; RWD = Radioactive waste disposed; CRU = Components
Caption for re-use; MFR = Materials for recycling; MER = Materials for energy recovery; EEE = Exported electrical energy; EET = Exported
thermal energy
RESULTS OF THE LCA – additional impact categories according to EN 15804+A2-optional:
1 m² floor covering
Indicator Unit A1-A3 A4 A5 B1 B2 C1 C2 C3/2 C3/3 C4/1 D D/1 D/2 D/3
[Disease -4.88E-
PM 1.96E-7 8.51E-9 6.71E-9 0.00E+0 6.84E-8 0.00E+04.71E-10 1.78E-8 1.94E-8 8.17E-9 0.00E+0 0.00E+0 -9.52E-9
Incidence] 10
[kBq U235-
IRP 9.04E-1 5.98E-4 2.76E-2 0.00E+0 6.78E-2 0.00E+0 3.31E-5 1.57E-2 2.59E-2 7.38E-3 -1.02E-2 0.00E+0 0.00E+0 -4.81E-3
Eq.]
ETP-fw [CTUe] 2.16E+2 2.29E+0 6.60E+0 3.60E-3 2.69E+0 0.00E+0 1.27E-1 1.49E+0 1.97E+0 3.98E+0 -1.67E-1 0.00E+0 0.00E+0-6.87E+0
-7.68E- -6.07E-
HTP-c [CTUh] 5.25E-9 4.64E-111.61E-100.00E+06.21E-100.00E+02.57E-126.84E-117.95E-111.79E-10 0.00E+0 0.00E+0
12 11
-2.95E-
HTP-nc [CTUh] 2.40E-7 2.75E-9 7.45E-9 2.60E-11 9.46E-9 0.00E+01.52E-10 4.99E-9 5.55E-9 1.50E-8 0.00E+0 0.00E+0 -3.07E-9
10
SQP [-] ND ND ND ND ND 0.00E+0 6.11E-2 6.49E-1 9.33E-1 2.84E-1 ND ND ND ND
PM = Potential incidence of disease due to PM emissions; IR = Potential Human exposure efficiency relative to U235; ETP-fw = Potential
Caption comparative Toxic Unit for ecosystems; HTP-c = Potential comparative Toxic Unit for humans (cancerogenic); HTP-nc = Potential
comparative Toxic Unit for humans (not cancerogenic); SQP = Potential soil quality index
No substantiated values can be given for the SQP indicator with the existing database.
The result figures given in module B2 refer to a period of 1 year because a reference service life is not declared.
They have to be multiplied by the assumed service life (in years) of the floor covering in the building under
consideration.
Disclaimer 1 – for the indicator “Potential Human exposure efficiency relative to U235”.
This impact category deals mainly with the eventual impact of low dose ionizingradiation on human health of the
nuclear fuel cycle. It does not consider effects due to possible nuclear accidents, occupational exposure nor due
to radioactive waste disposal in undergroundfacilities. Potential ionizing radiation from the soil, from radon and
from some construction materials is also not measured by this indicator.
Disclaimer 2 – for the indicators “abiotic depletion potential for non-fossil resources”, “abiotic depletion potential
for fossil resources”, “water (user) deprivation potential, deprivation-weighted water consumption”, “potential
comparative toxic unit for ecosystems”, “potential comparative toxic unit for humans – cancerogenic”, “Potential
comparative toxic unit for humans - not cancerogenic”, “potential soil quality index”.
The results of this environmental impact indicator shall be used with care as the uncertainties on these results are
high or as there is limited experienced with the indicator.
References
EN 1307 floor coverings – Environmental product declarations –
DIN EN 1307: 2014+A1:2016+A2:2018-05: Textile Product category rules
floor coverings - Classification
ISO 10874
EN 13501-1 DIN EN ISO 10874: 2012+A1:2021-04: Resilient,
DIN EN 13501-1:2019-05: Fire classification of textile and laminate floor coverings - Classification
construction products and building elements - Part 1:
Classification using data from reaction to fire tests ISO 14025
DIN EN /ISO 14025:2011-10/, Environmental labels
EN 14041 and declarations — Type III environmental
DIN EN 14041: 2018-05 and DIN EN 14041: 2008-05: declarations — Principles and procedures
Resilient, textile and laminate floor coverings -
Essential characteristics
ISO 14040
EN 15804 DIN EN ISO 14040:2006+A1:2020 Environmental
DIN EN 15804:2012+A2:2019 + AC:2021, management - Life cycle assessment - Principles and
Sustainability of construction works — Environmental framework
Product Declarations — Core rules for the product
category of construction products ISO 14044
DIN EN ISO 14044:2006+A1:2018+A2:2020
EN 16810 Environmental management - Life cycle assessment -
DIN EN 16810: 2017-08: Resilient, textile and laminate Requirements and guidelines
7 Environmental Product Declaration Interface – Superfloor II, Needled tiles with a total pile weight of 521 g/m2 and a
CQuest Bio backing
ISO 15686 GaBi database
ISO 15686: Buildings and constructed assets - GaBi Software-System and Database for Life Cycle
Service life planning Engineering, version 10.5 Sphera, Leinfelden-
ISO 15686-1: 2011-05: Part 1: General principles and Echterdingen, database version 2022-1
framework
ISO 15686-2: 2012-05: Part 2: Service life prediction PCR Part A
procedures Product Category Rules for Building-Related Products
ISO 15686-7: 2017-04: Part 7: Performance and Services Part A: Calculation Rules for the Life
evaluation for feedback of service life data Cycle Assessment and Requirements on the Project
from practice Report according to EN 15804+A2:2019, V1.2, Berlin:
ISO 15686-8: 2008-06: Part 8: Reference service life Institut Bauen und Umwelt e.V. (IBU), November 2021
and service-life estimation
PCR Part B
Regulation (EU) No. 305/2011 Product Category Rules for Building-Related Products
Regulation No. 305/2011 Construction Products and Services
Regulation (CPR) of the European Council and of the Part B: Requirements on the EPD for floor coverings,
European Parliament, April 2011 V1.2, Berlin: Institut Bauen und Umwelt e.V. (IBU),
February 2018
General Instructions for the IBU-EPD Program
General Instructions for the EPD-Program of the PRODIS
Institut Bauen und Umwelt e.V., The Preparation of Product Information System (PRODIS) of the
Environmental Product Declarations - EPDs, version European Carpet Industry, Gemeinschaft
2.0, Institut Bauen und Umwelt e.V., Berlin, January umweltfreundlicher Teppichboden e.V (GUT) and
2021, www.ibu-epd.de European Carpet and Rug Association
(ECRA), http://www.pro-dis.info
BNB, Nutzungsdauer von Bauteilen
Bewertungssystem Nachhaltiges Bauen (BNB), REACH
Nutzungsdauer von Bauteilen, Bundesministerium des Regulation (EC) No 1907/2006 of the European
Inneren, für Bau und Heimat, 24.02.2017 Parliament and of the Council of 18 December 2006
concerning the Registration, Evaluation, Authorisation
ECHA candidate list and Restriction of Chemicals (REACH), June 2017,
Candidate List of substances of very high concern last update: 08.07.2021
(SVHCs) for authorisation, 08.07.2021, European
Chemicals Agency (ECHA), Helsinki, Finland VDZ e.V.
Association of German Cement Works, Ed. Environ-
mental Data of the German Cement Industry 2020
ecoinvent
ecoinvent, Zurich, Switzerland, database version 3.7,
published September 2020
8 Environmental Product Declaration Interface – Superfloor II, Needled tiles with a total pile weight of 521 g/m2 and a
CQuest Bio backing
Publisher
Institut Bauen und Umwelt e.V. Tel +49 (0)30 3087748- 0
Hegelplatz 1 Fax +49 (0)30 3087748- 29
10117 Berlin Mail info@ibu-epd.com
Germany Web www.ibu-epd.com
Programme holder
Institut Bauen und Umwelt e.V. Tel +49 (0)30 - 3087748- 0
Hegelplatz 1 Fax +49 (0)30 – 3087748 - 29
10117 Berlin Mail info@ibu-epd.com
Germany Web www.ibu-epd.com
Author of the Life Cycle
Assessment Tel +49 (0)241 96843 410
Gemeinschaft umweltfreundlicher Fax +49 (0)241 96843 400
Teppichboden (GUT) e.V. Mail mail@gut-ev.de
Schönebergstraße 2 Web www.gut-ev.org
52068 Aachen
Germany
Owner of the Declaration
Interface Europe Manufacturing Tel +31 33 277 55 55
BV Fax +31 33 277 55 54
Industrielaan 15 Mail receptie@interface.com
3925ZG Scherpenzeel Web www.interface.com
Netherlands
