Environmental product declaration
In accordance with 14025 and EN15804+A2
Table S Ø500
Owner of the declaration: Program operator:
Fora Form AS The Norwegian EPD Foundation
Declaration number:
Table S Ø500
Registration number:
Declared unit:
1 pcs Issue date:
25.04.2023
This declaration is based on Product Category Rules:
CEN Standard EN 15804:2012+A2:2019 serves as core Valid to:
PCR
The Norwegian EPD Foundation EPD Software:
NPCR 026:2018 Part B for furniture
LCA.no EPD generator ID: 61188
1 / 12
General information
Product Owner of the declaration:
Table S Ø500 Fora Form AS
Contact person: Kåre Sætre
Phone: +47 700 46 000
e-mail: info@foraform.com
Program operator: Manufacturer:
Post Box 5250 Majorstuen, 0303 Oslo, Norway Fora Form AS
The Norwegian EPD Foundation
Phone: +47 23 08 80 00
web: post@epd-norge.no
Declaration number: Place of production:
Fora Form AS
Mosflatevegen
6154 Ørsta, Norway
This declaration is based on Product Category Rules: Management system:
CEN Standard EN 15804:2012+A2:2019 serves as core PCR NS-EN ISO 14001: 2015 No. 800406.NS-EN ISO 9001: 2015 No.
NPCR 026:2018 Part B for furniture 901268.NS-EN ISO 45001: 2018 No 907167.
Statement of liability: Organisation no:
The owner of the declaration shall be liable for the underlying 986 581 421
information and evidence. EPD Norway shall not be liable with respect
to manufacturer information, life cycle assessment data and
evidences.​
Declared unit: Issue date:
1 pcs Table S Ø500 25.04.2023
Declared unit (cradle to gate) with option: Valid to:
A1-A3,A4,A5,B1,B2,C1,C2,C3,C4,D
Year of study:
2023
Functional unit: Comparability:
Production of one table solution provided and maintained for a EPD of construction products may not be comparable if they not
period of 15 years. comply with EN 15804 and seen in a building context.
General information on verification of EPD from EPD tools: Development and verification of EPD:
Independent verification of data, other environmental information The declaration is created using EPD tool lca.tools ver EPD2022.03,
and the declaration according to ISO 14025:2010, § 8.1.3 and § 8.1.4. developed by LCA.no. The EPD tool is integrated in the company's
Individual​ third party verification of each EPD is not required when management system, and has been approved by EPD Norway.
the EPD tool is i) integrated into the company's environmental
management system, ii) the procedures for use of the EPD tool are Developer of EPD: Kåre Sætre
approved by EPDNorway, and iii)​ the proccess is reviewed annualy.
Reviewer of company-specific input data and EPD: Stig Robert
See Appendix G of EPD-Norway's General Programme Instructions
Sporstøl
for further information on EPD tools.
Verification of EPD tool: Approved:
Independent third party verification of the EPD tool, background data
and test-EPD in accordance with EPDNorway's procedures and
guidelines for verification and approval of EPD tools.
Third party verifier:
Elisabet Amat Håkon Hauan, CEO EPD-Norge
(no signature required)
2 / 12
Product
Product description:
S tables are smal tables designed by the duo Anderssen & Voll. With its effortless elegant expression, the table is suitable for most places where a
smaller table top is needed.The table series consists of three variants , S,R ,L
S table that has circular geometry. R table that has rectangular geometry. L table with rectangular geometry and power outlet in the base
The table series makes every Chair into a work station, and the L series even offers electrical sockets for uncomplicated charging. Today's Offices
has many different ways and Places to work. The L, R and S table makes working in any sofa or chair effortless and user-friendly.
Table top 25 mm solid oak with chamfered edge and rounded corners. Standard configuration is in black stained oak with the base is lacquered in
the Sahara Collection from Jotun, which provides a textured surface.
Please note that the L and S table are also avaliable as a fixed version for assembly on the Senso sofa.
Product specification
Materials kg %
Metal - Steel 5,60 59,01
Paint, solvent-based 0,15 1,58
Powder coating 0,04 0,42
Wood - Solid oak 3,70 38,99
Total 9,49
Packaging kg %
Packaging - Cardboard 2,00 100,00
Total incl. packaging 11,49
Technical data:
Table S Ø500 Oak
Height 600 mm
Dia. 500 mm
Weight 9,65 kg.
Table S Ø340 Oak
Height 600 mm
Dia. 340 mm
Weight 7,4 kg.
Market:
Worldwide
Reference service life, product
15 years
Reference service life, building
LCA: Calculation rules
Declared unit:
1 pcs Table S Ø500
Cut-off criteria:
All major raw materials and all the essential energy is included. The production processes for raw materials and energy flows with very small
amounts (less than 1%) are not included. These cut-off criteria do not apply for hazardous materials and substances.
Allocation:
The allocation is made in accordance with the provisions of EN 15804. Incoming energy and water and waste production in-house is allocated
equally among all products through mass allocation. Effects of primary production of recycled materials is allocated to the main product in which
the material was used. The recycling process and transportation of the material is allocated to this analysis.
Data quality:
Specific data for the product composition are provided by the manufacturer. They represent the production of the declared product and were
collected for EPD development in the year of study. Background data is based on registered EPDs according to EN 15804, Ostfold Research
databases, ecoinvent and other LCA databases. The data quality of the raw materials in A1 is presented in the table below.​
3 / 12
Materials Source Data quality Year
Metal - Steel ecoinvent 3.6 Database 2019
Packaging - Cardboard ecoinvent 3.6 Database 2019
Paint, solvent-based ecoinvent 3.6 Database 2019
Powder coating Ecoinvent 3.6 Database 2019
Wood - Solid oak modified ecoinvent 3.6 Database 2019
4 / 12
System boundaries (X=included, MND=module not declared, MNR=module not relevant)
Construction Beyond the system
Product stage Use stage End of life stage
installation stage boundaries
A1 A2 A3 A4 A5 B1 B2 B3 B4 B5 B6 B7 C1 C2 C3 C4 D
X X X X X X X MND MND MND MND MND X X X X X
System boundary:
Additional technical information:
We want you to enjoy your furniture for many years to come. If you follow our advice in this Quality and Maintenance Manual you contribute to
prolonged life of your furniture. We only use environmentally friendly materials and processes in our manufacturing unit in Ørsta Norway. Our goal
is to manufacture furniture that can last for generations. All furniture made by Fora Form are made of FSC certified wood, manufactured according
to ISO 14001, and has an EPD on all products. This ensures sustainability and a “cradle to cradle” philosophy. We actively work to reduce waste. All
packing materials and waste are being recycled according to Norsk Gjenvinning.
Norwegian and Swedish Møbelfakta are accredited test facilities where furniture quality, strength, durability, flammability, safety, emissions and
materials are tested and documented. A piece of furniture, which lives up to the three areas of requirements of Møbelfakta, has undergone
extensive testing, is produced according to ethical guidelines and has been approved according to environmental requirements. Møbelfakta is a
guarantee of high quality products. Almost all of Fora Forms collection is Møbelfakta approved.
Fora Form are ISO 9001 quality management,ISO 14001 environmental management and ISO 45001 occupational health and safety management
certified. Sustainability is important for Fora Form.
We continuously work to sort and reduce our waste, and collaborate with Norsk Gjenvinning and Grønt Punkt (Green Dot Norway plc) regarding
recycling of used packing materials. All wood is FSC certified.
Our manufacturing unit in Ørsta use electricity that is 100% originated from renewable sources.
Transportation to an average customer in Oslo is 540 km
waR slairetam tropsnarT gnirutcafunaM tropsnarT ylbmessA e​sU ecnanetniaM riapeR tnemecalpeR tnemhsibrufeR lanoitarepO ygrene esu lanoitarepO esu retaw -eD noitcurtsnoc noitilomed tropsnarT etsaW gnissecorp lasopsiD -yrevoceR-esueR laitnetop-gnilcyceR
5 / 12
LCA: Scenarios and additional technical information
The following information describe the scenarios in the different modules of the EPD.
Capacity utilisation Value
Transport from production place to user (A4) Distance (km) Fuel/Energy Consumption Unit
(incl. return) % (Liter/tonne)
Truck, 16-32 tonnes, HVO, EURO 6 (kgkm) 36,7 % 540 0,043 l/tkm 23,22
Assembly (A5) Unit Value
Waste, packaging, corrugated board box, to
kg 2,00
average treatment (kg)
Maintenance (B2) Unit Value
Water, tap water (kg) kg/DU 1,00
Waste processing (C3) Unit Value
Waste treatment per kg Non-hazardous waste,
kg 0,04
incineration with fly ash extraction - C3 (kg)
Waste treatment per kg Scrap steel, incineration
kg 5,60
with fly ash extraction (kg)
Waste treatment per kg Wood, incineration with
kg 3,70
fly ash extraction (kg)
Waste, materials to recycling (kg) kg 1,90
Disposal (C4) Unit Value
Landfilling of ashes and residues from
kg 3,70
incineration of Scrap steel (kg)
Landfilling of ashes from incineration of Non-
hazardous waste, process per kg ashes and kg 0,01
residues - C4 (kg)
Landfilling of ashes from incineration of Wood,
kg 0,04
process per kg ashes and residues (kg)
Benefits and loads beyond the system
Unit Value
boundaries (D)
Substitution of electricity, in Norway (MJ) MJ 2,60
Substitution of primary steel with net scrap (kg) kg 1,52
Substitution of thermal energy, district heating, in
MJ 39,29
Norway (MJ)
6 / 12
LCA: Results
The LCA results are presented below for the declared unit defined on page 2 of the EPD document.
Environmental impact
Indicator Unit A1-A3 A4 A5 B1 B2 C1 C2 C3 C4 D
GWP-total
kg CO2 -
2,98E+01 2,45E-01 3,43E+00 0 3,46E-04 0 0 6,33E+00 4,15E-02 -1,91E+00
eq
GWP-fossil
kg CO2 -
3,86E+01 2,44E-01 3,24E-02 0 3,43E-04 0 0 1,65E-01 4,15E-02 -1,90E+00
eq
GWP-biogenic
kg CO2 -
-9,07E+00 4,13E-04 3,40E+00 0 2,16E-06 0 0 6,17E+00 3,12E-05 -1,39E-03
eq
GWP-luluc
kg CO2 -
2,91E-01 3,80E-04 1,07E-05 0 5,59E-07 0 0 1,61E-05 1,26E-05 -8,60E-03
eq
kg
ODP CFC11 - 3,49E-06 5,03E-08 6,83E-09 0 3,00E-11 0 0 6,91E-09 1,29E-08 -1,66E-02
eq
mol H+
AP 2,72E-01 1,71E-03 1,53E-04 0 2,00E-06 0 0 7,85E-04 2,94E-04 -1,02E-02
-eq
EP-FreshWater kg P -eq 2,73E-03 8,96E-06 2,66E-07 0 2,74E-08 0 0 1,70E-06 4,13E-07 -1,23E-04
EP-Marine kg N -eq 4,22E-02 4,53E-04 5,07E-05 0 3,18E-07 0 0 3,55E-04 1,05E-04 -2,33E-03
mol N -
EP-Terrestial 4,52E-01 5,06E-03 5,49E-04 0 3,70E-06 0 0 3,79E-03 1,16E-03 -2,42E-02
eq
kg
POCP NMVOC 1,52E-01 1,85E-03 1,58E-04 0 1,16E-06 0 0 9,77E-04 3,35E-04 -1,02E-02
-eq
ADP- kg Sb -
1,44E-03 2,97E-05 7,87E-07 0 9,59E-09 0 0 3,86E-07 7,21E-07 -3,11E-05
minerals&metals1 eq
ADP-fossil1 MJ 4,86E+02 5,16E+00 4,53E-01 0 5,86E-03 0 0 6,45E-01 9,53E-01 -1,73E+01
WDP1 m3 1,74E+03 1,53E+01 5,74E-01 0 1,04E-01 0 0 1,55E+00 1,86E+00 4,62E+01
GWP total = Global Warming Potential total; GWP fossil = Global Warming Potential fossil fuels ; GWP biogenic = Global Warming Potential biogenic; GWP luluc =
Global W Potential land use change; ODP = Ozone Depletion; AP = Acidification; EP freshwater = Eutrophication aquatic freshwater; EP = marine Eutrophication aquatic
marine; EP = terrestrial Eutrophication terrestrial ;POCP = Photochemical zone formation; ADPE = Abiotic Depletion Potential minerals and metals; ADPF = Abiotic
Depletion Potential fossil fuels;
"Reading example: 9,0 E-03 = 9,0*10-3 = 0,009"
*INA Indicator Not Assessed
1. The results of this environmental impact indicator shall be used with care as the uncertainties on these results are high or as there is limited experienced with the
indicator
Remarks to environmental impacts
The product contains no substances given by the REACH Candidate list or the Norwegian priority list.
7 / 12
Additional environmental impact indicators
Indicator Unit A1-A3 A4 A5 B1 B2 C1 C2 C3 C4 D
PM Disease incidence 2,79E-06 5,66E-08 2,26E-09 0 1,70E-11 0 0 1,58E-08 5,40E-09 -2,53E-07
IRP2 kgBq U235 -eq 1,80E+00 1,69E-02 1,94E-03 0 4,05E-05 0 0 1,55E-03 3,81E-03 -1,48E-02
ETP-fw1 CTUe 2,78E+03 7,54E+00 6,04E-01 0 6,35E-03 0 0 3,11E+00 5,60E-01 -1,11E+02
HTP-c1 CTUh 1,65E-07 0,00E+00 1,80E-11 0 1,00E-12 0 0 4,01E-10 1,90E-11 -8,37E-09
HTP-nc1 CTUh 2,45E-06 1,26E-08 7,58E-10 0 2,10E-11 0 0 7,85E-09 5,30E-10 1,58E-07
SQP1 dimensionless 5,14E+02 9,63E+00 3,04E-01 0 1,64E-03 0 0 1,24E-01 2,08E+00 -2,28E+01
PM = Particulate Matter emissions; IRP = Ionizing radiation – human health; ETP-fw = Eco toxicity – freshwater; HTP-c = Human toxicity – cancer effects; HTP-nc =
Human toxicity – non cancer effects; SQP = Soil Quality (dimensionless)
"Reading example: 9,0 E-03 = 9,0*10-3 = 0,009"
*INA Indicator Not Assessed
1. The results of this environmental impact indicator shall be used with care as the uncertainties on these results are high or as there is limited experienced with the
indicator
2. This impact category deals mainly with the eventual impact of low dose ionizing radiation on human health of the nuclear fuel cycle. It does not consider effects due
to possible nuclear accidents, occupational exposure nor due to radioactive waste disposal in underground facilities. Potential ionizing radiation from the soil, from
radon and from some construction materials is also not measured by this indicator.
8 / 12
Resource use
Indicator Unit A1-A3 A4 A5 B1 B2 C1 C2 C3 C4 D
PERE MJ 1,18E+02 2,34E-01 7,45E-03 0 7,95E-04 0 0 2,69E-02 1,76E-02 -2,13E+01
PERM MJ 6,82E+01 0,00E+00 -1,64E+01 0 0,00E+00 0 0 -5,18E+01 0,00E+00 0,00E+00
PERT MJ 1,86E+02 2,34E-01 -1,64E+01 0 7,95E-04 0 0 -5,17E+01 1,76E-02 -2,13E+01
PENRE MJ 4,87E+02 5,16E+00 4,53E-01 0 5,87E-03 0 0 6,50E-01 9,54E-01 -1,73E+01
PENRM MJ 0,00E+00 0,00E+00 0,00E+00 0 0,00E+00 0 0 0,00E+00 0,00E+00 0,00E+00
PENRT MJ 4,87E+02 5,16E+00 4,53E-01 0 5,87E-03 0 0 6,50E-01 9,54E-01 -1,73E+01
SM kg 1,84E+00 0,00E+00 0,00E+00 0 0,00E+00 0 0 0,00E+00 0,00E+00 7,92E-01
RSF MJ 3,47E-01 7,60E-03 2,47E-04 0 6,39E-05 0 0 5,74E-04 4,67E-04 5,69E-02
NRSF MJ 1,64E+00 2,62E-02 1,02E-03 0 6,30E-05 0 0 0,00E+00 3,41E-02 5,66E-01
FW m3 3,04E-01 2,11E-03 2,14E-04 0 1,01E-03 0 0 1,06E-03 8,59E-04 -2,77E-02
PERE Use of renewable primary energy excluding renewable primary energy resources used as raw materials; PERM Use of renewable primary energy resources used as
raw materials; PERT Total use of renewable primary energy resources; PENRE Use of non renewable primary energy excluding non-renewable primary energy resources
used as raw materials; PENRM Use of non renewable primary energy resources used as raw materials; PENRT Total use of non renewable primary energy resources; SM
Use of secondary materials; RSF Use of renewable secondary fuels; NRSF Use of non renewable secondary fuels; FW Use of net fresh water
"Reading example: 9,0 E-03 = 9,0*10-3 = 0,009"
*INA Indicator Not Assessed
9 / 12
End of life - Waste
Indicator Unit A1-A3 A4 A5 B1 B2 C1 C2 C3 C4 D
HWD kg 2,74E-01 7,25E-04 2,00E-03 0 1,11E-06 0 0 0,00E+00 3,72E+00 -8,85E-03
NHWD kg 1,20E+01 7,68E-01 2,26E-02 0 7,12E-05 0 0 0,00E+00 3,35E-02 -7,61E-01
RWD kg 1,85E-03 2,07E-05 2,99E-06 0 3,43E-08 0 0 0,00E+00 5,85E-06 -1,24E-05
HWD = Hazardous waste disposed; NHWD = Non-hazardous waste disposed; RWD = Radioactive waste disposed;
"Reading example: 9,0 E-03 = 9,0*10-3 = 0,009"
*INA Indicator Not Assessed
End of life - Output flow
Indicator Unit A1-A3 A4 A5 B1 B2 C1 C2 C3 C4 D
CRU kg 0,00E+00 0,00E+00 0,00E+00 0 0,00E+00 0 0 0,00E+00 0,00E+00 0,00E+00
MFR kg 0,00E+00 0,00E+00 1,86E+00 0 0,00E+00 0 0 1,90E+00 0,00E+00 7,93E-01
MER kg 0,00E+00 0,00E+00 2,72E-06 0 0,00E+00 0 0 9,34E+00 0,00E+00 5,04E-04
EEE MJ 0,00E+00 0,00E+00 1,14E-01 0 0,00E+00 0 0 2,73E+00 0,00E+00 -5,75E-04
EET MJ 0,00E+00 0,00E+00 1,73E+00 0 0,00E+00 0 0 4,13E+01 0,00E+00 -8,70E-03
CRU = Components for re-use; MFR = Materials for recycling; MER = Materials for energy recovery; EEE = Exported energy electrical; EET = Exported energy Thermal;
"Reading example: 9,0 E-03 = 9,0*10-3 = 0,009"
*INA Indicator Not Assessed
Biogenic Carbon Content
Indicator Unit At the factory gate
Biogenic carbon content in product kg C 1,68E+00
Biogenic carbon content in accompanying packaging kg C 9,26E-01
Note: 1 kg biogenic carbon is equivalent to 44/12 kg CO2
10 / 12
Additional Norwegian requirements
Greenhouse gas emissions from the use of electricity in the manufacturing phase
National production mix from import, low voltage (production of transmission lines, in addition to direct emissions and losses in grid) of applied
electricity for the manufacturing process (A3).
Electricity mix Data source Amount Unit
Electricity, European average (kWh) ecoinvent 3.6 428,03 g CO2-eq/kWh
Dangerous substances
No substances given by the REACH Candidate list or the Norwegian priority list are intentionally added to the product.
Indoor environment
Our furniture doesn't contain any substanses that effect indoor clima, and therefore satisfies the requirements for low emissions.
Additional Environmental Information
Environmental impact indicators EN 15804+A1 and NPCR Part A v2.0
Indicator Unit A1-A3 A4 A5 B1 B2 C1 C2 C3 C4 D
GWP kg CO2 -eq 1,95E+01 2,34E-01 3,22E-02 0 3,34E-04 0 0 1,17E+01 2,00E-03 -1,80E+00
ODP kg CFC11 -eq 1,73E-06 3,77E-08 5,50E-09 0 3,50E-11 0 0 3,45E-09 2,06E-10 -7,77E-08
POCP kg C2H4 -eq 7,61E-03 8,56E-05 4,59E-06 0 1,08E-07 0 0 1,42E-05 2,46E-07 -1,31E-03
AP kg SO2 -eq 1,38E-01 9,50E-04 8,22E-05 0 1,56E-06 0 0 4,07E-04 3,70E-06 -7,66E-03
EP kg PO43- -eq 1,34E-02 1,41E-04 1,41E-05 0 1,89E-07 0 0 1,40E-04 4,90E-07 -1,33E-03
ADPM kg Sb -eq 9,44E-04 2,97E-05 7,87E-07 0 9,59E-09 0 0 1,90E-07 1,33E-08 -3,11E-05
ADPE MJ 2,23E+02 4,73E+00 4,42E-01 0 3,81E-03 0 0 3,69E-01 2,07E-02 -1,79E+01
GWPIOBC kg CO2 -eq 3,99E+01 2,45E-01 0,00E+00 0 3,46E-04 0 0 5,51E+00 2,00E-03 -2,74E+00
GWP Global warming potential; ODP Depletion potential of the stratospheric ozone layer; POCP Formation potential of tropospheric photochemical oxidants; AP
Acidification potential of land and water; EP Eutrophication potential; ADPM Abiotic depletion potential for non fossil resources; ADPE Abiotic depletion​ potential for
fossil resources; GWP-IOBC/GHG Global warming potential calculated according to the principle of instantanious oxidation (except emissions and uptake of biogenic
carbon)
Variants and Options
Key environmental indicators (A1-A3) for variants of this EPD
Variants Weight (kg) GWPtotal (kg CO2 -eq) Total energy consumption (MJ) Secondary material (%)
Table S Ø340 9,40 32,63 552,19 56,00
Key Environmental Indicators
Indicator Unit A1-A3 A4 A1-C4 A1-D
GWPtotal kg CO2 -eq 29,79 0,24 39,84 37,93
Total energy consumption MJ 606,79 5,43 614,37 576,40
Secondary materials % 56,00
11 / 12
Bibliography
ISO 14025:2010 Environmental labels and declarations - Type III environmental declarations - Principles and procedures.
ISO 14044:2006 Environmental management - Life cycle assessment - Requirements and guidelines.
EN 15804:2012+A2:2019 Environmental product declaration - Core rules for the product category of construction products.
ISO 21930:2017 Sustainability in buildings and civil engineering works - Core rules for environmental product declarations of construction
products.
ecoinvent v3, Allocation, cut-off by classification, Swiss Centre of Life Cycle Inventories.
Iversen et al., (2021) eEPD v2021.09 Background information for EPD generator tool system verification, LCA.no Report number: 07.21
Ruud et al., (2023) EPD generator for NPCR026 Part B for Furniture - Background information for EPD generator application and LCA data,
LCA.no report number 01.23
NPCR Part A: Construction products and services. Ver. 2.0. March 2021, EPD-Norge.
NPCR 026 Part B for Furniture. Ver. 2.0 March 2022, EPD-Norge.
Program operator and publisher Phone: +47 23 08 80 00
The Norwegian EPD Foundation e-mail: post@epd-norge.no
Post Box 5250 Majorstuen, 0303 Oslo, Norway web: www.epd-norge.no
Owner of the declaration: Phone: +47 700 46 000
Fora Form AS e-mail: info@foraform.com
Mosflatevegen, 6154 Ørsta web: www.foraform.no
Author of the Life Cycle Assessment Phone: +47 916 50 916
LCA.no AS e-mail: post@lca.no
Dokka 6B, 1671 web: www.lca.no
Developer of EPD generator Phone: +47 916 50 916
LCA.no AS e-mail: post@lca.no
Dokka 6B,1671 Kråkerøy web: www.lca.no
ECO Platform web: www.eco-platform.org
ECO Portal web: ECO Portal
12 / 12
