Environmental Product
Declaration
In accordance with ISO 14025 and EN 15804 +A2
Owner of the declaration: Tegra 400 and 425
Norsk Wavin AS
Program holder and publisher:
Plastic inspection chamber made
The Norwegian EPD foundation
of polypropylene according to DIN
EN 13598-2.
Declaration number:
NEPD-3767-2675-EN
Manufacturer
Registration number:
Wavin Polska S.A.
NEPD-3767-2675-EN
Issue date: 03.10.2022
The Norwegian Valid to: 03.10.2027
EPD Foundation
Ver2-101122
General information
Product:
Owner of the declaration:
Tegra 400 and 425
Norsk Wavin AS
Contact person: Matteo Tagliaferri
Program Operator:
Phone: +31 +31623193684
The Norwegian EPD Foundation
e-mail: matteo.tagliaferri@wavin.com
Post Box 5250 Majorstuen, 0303 Oslo, Norway
Tlf: +47 23 08 80 00
Manufacturer:
e-mail: post@epd-norge.no
Wavin Polska S.A.
Dobieżyńska 43, 64-320 Buk, Poland
Declaration Number:
Phone: +48 61 891 10 00
NEPD-3767-2675-EN
e-mail: kontakt_pl@wavin.pl
This declaration is based on Product
Place of production:
Category Rules:
Dobieżyńska 43, 64-320 Buk, Poland
CEN standard EN 15804:2012+A2:2019 serves as
core PCR, supplied with NPCR Part A, Version 2.0.
Management system:
EN ISO 9001:2015 and EN ISO 14001:2015
Statements:
The owner of the declaration shall be liable for the
Organisation no:
underlying information and evidence. EPD
823355092
Norway shall not be liable with respect to
manufacturer, life cycle assessment data and
Issue date:
evidences.
03.10.2022
Declared unit:
Valid to:
1 kg Tegra 400/425
03.10.2027
Declared unit with option:
Year of study:
A1,A2,A3,A4,A5,C1,C2,C3,C4,D
2020
Functional unit:
Comparability:
Not applicable.
EPDs from other programmes than the Norwegian
Verification: EPD foundation may not be comparable.
Independent verification of the declaration and
data, according to ISO14025:2010 The EPD has been worked out by:
internal external Lisa Overmars and Emma Thunnissen,
Ecochain Technologies
Harry van Ewijk, SGS Search
Independent verifier approved by EPD Norway
Approved (Manager of EPD Norway)
EPD for the best environmental decision 2
Product
Product description:
Inspection chamber for municipal industrial and domestic drainage system for foul and
rainwater systems. Tegra 400 PP and 425 PP can be installed in heavy traffic area according to
LM1 (DIN EN 1991-2/NA) former SLW60. Smooth wall pipe and X-Stream pipes can be
connected directly. Installation depths up to 6.0 m, in groundwater max. 5.0m, for Tegra 400
max 3.0m, are possible. Tegra is equipped with an integrated flexible ball joints to adjust change
in directions and gradients.
Product specification:
A typical composition of the Tegra 400/425, including packaging, covered by this EPD is as
follows:
Materials %
Polypropylene (PP) 51,0%
Additives 1,7%
Packaging 43,4%
Rubber seal 3,8%
The specifications of the products covered in this EPD are:
• Diameter - DN/ID-OD 400, 425
• Material - Polypropylene (PP)
• Chemical resistance - Sewer environment
• Max. installation depth - 6 m
• Max. installation depth in groundwater – Tegra 400: 3m, Tegra 425: 5m
• Traffic load - up to SLW 60
• Cover class - A15-D400
Technical data:
The declared unit of this EPD is 1 kg Tegra 400/425. The results per kg are based on the
product ‘Tegra 425 PP Straight DN160 SW’ (‘base product’). The Table below provides the
products covered with this EPD. The selected base product is representative for all products
described in this Table; deviations of the LCA results of the other products compared to the base
product are not more than 10%.
The list below provides the mass per piece (including packaging). These masses should be used
to calculate the LCA results per 1 piece, by multiplying the results of all modules, except ‘A5 –
installation’, presented on page 9-12, with the weight specified below. The LCA results of ‘A5 –
installation’ should be calculated from the LCA results presented on pages 7-8 under ‘addtional
technical information’.
EPD for the best environmental decision 3
Mass Mass
Product Product
(kg/pc) (kg/pc)
Tegra 425 PP Straight DN110 SW 16,06 Tegra 425 PP T 90° DN160 SW 18,10
Tegra 425 PP Straight DN160 SW 16,54 Tegra 400 PP Bend 90° DN200 SW 18,20
Tegra 425 PP Bend 150° DN160 SW 16,54 Tegra 425 PP Straight DN200 X- 18,31
Tegra 425 PP Bend 90° DN160 SW 16,54 Tegra 400 PP Straight DN200 SW 18,32
Tegra 425 PP Cross 90° DN110 SW 16,77 Tegra 425 PP Cross 90° DN150 X- 18,33
Tegra 400 PP Bend 150° DN160 SW 16,82 Tegra 400 PP Bend 150° DN200 SW 18,34
Tegra 400 PP Bend 120° DN160 SW 16,82 Tegra 400 PP Bend 120° DN200 SW 18,34
Tegra 400 PP Bend 90° DN160SW 16,82 Tegra 425 PP Cross 90° DN160 SW 18,49
Tegra 400 PP Straight DN160 SW 16,92 Tegra 425 PP Bend 90° DN200 SW 18,63
Tegra 425 PP Straight DN150 X- 17,29 Tegra 425 PP Bend 150° DN200 SW 18,69
Tegra 425 PP Straight DN160 SW 17,30 Tegra 425 PP Bend 120° DN200 SW 18,69
Tegra 425 PP Bend 150° DN160 SW 17,30 Tegra 425 PP Straight DN200 SW 18,72
Tegra 425 PP Bend 120° DN160 SW 17,30 Tegra 425 PP Straight DN200 OR 18,73
Tegra 425 PP Bend 90° DN160 SW 17,30 Tegra 425 PP T 90° DN200 SW 20,06
Tegra 425 PP T 90° DN160 SW AU 17,33 Tegra 425 PP T 90° DN200 OR 20,08
Tegra 425 PP Cross 90° DN160 SW 17,73 Tegra 400 PP Cross 90° DN200 SW 20,94
Tegra 400 PP Cross 90° DN160 SW 18,06 Tegra 425 PP Cross 90° DN200 SW 21,36
Market:
Europe, but the EPD is specific for Nordic countries.
Reference service life, product:
100 years
Reference service life, building:
LCA: Calculation rules
Declared unit:
1 kg Tegra 400/425
Data quality:
For module A1, specific data for product compositions as provided by the manufacturer are
used. For module A2, transportation data of the raw materials used to the production site was
collected. For module A3, energy consumption and waste production data was collected for
production year 2020. The used background processes are derived from Ecoinvent 3.6.
Allocation:
Allocation was carried out in accordance with the povisions of the EN15804. All manufacturing
inputs (energy and auxiliary materials) at production site level are allocated to different
production processes, followed by allocation of the production processes to the products that
are produced using these processes through mass allocation. No secondary materials have been
used in the production process.
EPD for the best environmental decision 4
System boundary:
Modules A1-A5 and C1-D are included. The figure below shows a (simplified) process tree.
Cut-off criteria:
All relevant inputs and outputs - like emissions, energy and materials - have been taken into
account in this LCA. In accordance with EN15804, the total neglected input flows per module
does not exceed 5% of energy usage and mass.
EPD for the best environmental decision 5
LCA: Scenarios and additional technical information
The following information describe the scenarios in the different modules of the EPD.
Transport from production place to assembly/user (A4)
The transportation distance from Buk to Oslo was considerd.
Capacity utilisation
Type Type of vehicle Distance KM Fuel/Energy consumption
(incl. return) %
Truck 50% Unspecified 1086 0,027 l diesel/tkm
Boat 50% Ferry 113 0,0295 kg heavy fuel oil/tkm
Assembly (A5)
Product losses of 2% are considered. This product is used underground, therefore use of an
excavator, soil transport, and a gravel foundation are necessary. For the foundation, gravel is
used; this gravel is assumed to be transported for 150 km. The excavation of the soil is
performed with a hydraulic digger. It is assumed that most of the soil is backfilled; however, the
soil replaced by the gravel foundation and the pipe is assumed to be transported elsewhere
(150 km). The compation of the soil is considered negligible. The dimensions of the trench are
dependent on the diameter of the product; for this reason, different scenarios were devised.
Unit Value
Material loss kg 0,02
Packaging waste kg 0,434
1 piece of Tegra 1 piece of Tegra
Unit
400 425
l/tonne excavated
Energy consumption of excavated volume 0.13 0.13
(diesel)
Excavated mass, total kg 1920.00 2167.50
Excavated mass transported to deposite kg 368.00 415.44
Transport distance from construction site km 150.00 150.00
Refilling mass (dirt + gravel foundation) kg 1595.20 1800.83
Transport distance for refilling mass to
km
construction site 1920.00 2167.50
kWh or l/tonne
Energy used for compaction - -
compacted
End of Life (C1, C3, C4)
Demolition is done manually, and therefore no energy is needed. The considered waste
treatment for the pipe is 70% recycling, 20% incineration and 10% landfill.
Unit Value
Collected as mixed construction waste kg 0,57
Reuse kg 0
Recycling kg 0,37
EPD for the best environmental decision 6
Energy recovery kg 0,14
To landfill kg 0,06
Transport to waste processing (C2)
The considered distances are 50 km to landfill, 100 km for energy recovery, and 250 km for
recycling.
Capacity utilisation
Type Type of vehicle Distance KM Fuel/Energy consumption
(incl. return) %
Truck 50% Unspecified 192,0 0,027 l diesel/tkm
Benefits and loads beyond the system boundaries (D)
For the PP and additives, 0,67 kg of saved virgin PP was considered per kg material recycled
(total of A5 en C3). For the rubber seal, 0,67 kg of saved virgin EPDM was considered per kg
rubber seal recycled. The 67% is the considered quality factor, which means that the product is
at least three times recyclable. The benefits from exported energy were calculation from the
energy efficiencies for Nothern countries reported by CEWEP, which is equal to an electrical
efficiency of 11,0%, and a thermal efficiency of 72,6%. Energy recovery from all materials
(including rubber gasket and packaging) was considered. Substition of Norwegian electricity
mix and district heating mix was assumed.
Unit Value
Saving of virgin PP kg 0,25
Saving of virgin EPDM kg 0,002
Substition of electric energy MJ 0,58
Subsitition of thermal energy MJ 3,82
Additional technical information
Although most of this EPD can be scaled with the weight of the inspection chamber, this is not
the case for module A5 which scales with the diameter of the product. For each applicable
diameter, a scenario for installation of 1 piece of product was established. The results of these
scenarios per diameter are described in the tables below.
To calculate the results for a specific product, the masses per piece, as described on page 3-4
(under technical data) should be used to calculate the LCA results per 1 piece, combined with
the data in the tables below. This should be done by multiplying the LCA results presented on
page 9-12 of all modules, except ‘A5 – installation’, with the mass per piece. The LCA results of
A5 – installation should be calculated from the LCA results presented in the table below.
Impact Category/Parameter Installation Tegra 400 Installation Tegra 425
GWP-total 8.86E+00 1.00E+01
GWP-fossil 8.85E+00 9.99E+00
GWP-biogenic 7.20E-03 8.13E-03
GWP-LULUC 3.04E-03 3.43E-03
ODP 2.02E-06 2.28E-06
AP 5.30E-02 5.99E-02
EP-freshwater 7.33E-05 8.27E-05
EPD for the best environmental decision 7
EP-marine 1.94E-02 2.19E-02
EP-terrestial 2.14E-01 2.41E-01
POCP 6.08E-02 6.86E-02
ADP-M&M 2.23E-04 2.51E-04
ADP-fossil 1.35E+02 1.53E+02
WDP 4.93E-01 5.57E-01
PM 9.00E-07 1.02E-06
IRP 5.98E-01 6.75E-01
ETP-fw 1.09E+02 1.23E+02
HTP-c 4.01E-09 4.53E-09
HTP-nc 1.29E-07 1.46E-07
SQP 1.12E+02 1.26E+02
RPEE 2.31E+00 2.61E+00
RPEM 0.00E+00 0.00E+00
TPE 2.31E+00 2.61E+00
NRPE 1.43E+02 1.62E+02
NRPM 0.00E+00 0.00E+00
TRPE 1.43E+02 1.62E+02
SM 0.00E+00 0.00E+00
RSF 0.00E+00 0.00E+00
NRSF 0.00E+00 0.00E+00
W 7.64E-02 8.62E-02
HW 3.47E-04 3.92E-04
NHW 7.86E+00 8.87E+00
RW 9.21E-04 1.04E-03
CR 0.00E+00 0.00E+00
MR 0.00E+00 0.00E+00
MER 0.00E+00 0.00E+00
EEE 0.00E+00 0.00E+00
ETE 0.00E+00 0.00E+00
LCA: Results
The LCA results are presented below for the declared unit defined on page 2 of the EPD
document. Recalculation to results per piece can be done based on the technical data specified
on page 3 and 4.
EPD for the best environmental decision 8
System boundaries (X=included, MND= module not declared, MNR=module not
relevant)
Benefits
& loads
Assembly
Product stage Use stage End of life stage beyond
stage
system
boundary
s la ir e wta am R tr o p s n a r T g n ir u tc a fu n a M tr o p s n a r T y lb m e s s A e s U e c n a n e tn ia M r ia p e R tn e m e c a lp e R tn e m h s ib r u fe R la n o iy tag rr
eee pns Ou
e la n o itar re
ete
a
ps
w
Ou
n
on io
tcit ui rlo
tsm n ee od
c
-
tr o p s n a r T
g
n is s ee tc so ar Wp la s o p s iD
g
yn
r
eil
v
ec
soy ucc eee RR
---
la itn e to p
D R
A1 A2 A3 A4 A5 B1 B2 B3 B4 B5 B6 B7 C1 C2 C3 C4 D
X X X X X MND MND MND MND MND MND MND X X X X X
Core environmental impact indicators
A5 – insta-
Indicator Unit A1-A3 A4 A5 - other C1 C2 C3 C4 D
llation
GWP-total kg CO2 eq. 4,77E-01 8,11E-02 5,78E-01 1,01E+00 0,00E+00 1,43E-02 5,22E-01 6,97E-03 -8,53E-01
GWP-fossil kg CO2 eq. 1,43E+00 8,11E-02 5,77E-01 5,28E-02 0,00E+00 1,43E-02 5,22E-01 6,98E-03 -8,52E-01
GWP-biogenic kg CO2 eq. -9,51E-01 4,38E-05 4,70E-04 9,56E-01 0,00E+00 8,68E-06 -5,42E-04 6,14E-06 -7,44E-04
GWP-LULUC kg CO2 eq. 9,40E-04 3,04E-05 1,98E-04 2,28E-05 0,00E+00 5,06E-06 7,78E-05 1,21E-07 -5,75E-04
kg CFC11
ODP 8,31E-08 1,85E-08 1,32E-07 2,88E-09 0,00E+00 3,30E-09 1,03E-08 1,76E-10 -5,32E-08
eq.
AP mol H⁺ eq. 6,00E-03 6,37E-04 3,46E-03 1,72E-04 0,00E+00 8,15E-05 4,40E-04 4,22E-06 -2,69E-03
EP-freshwater kg P eq. 3,04E-05 6,38E-07 4,78E-06 7,41E-07 0,00E+00 1,23E-07 2,35E-06 5,76E-09 -1,38E-05
EP-marine kg N eq. 1,11E-03 2,05E-04 1,26E-03 4,09E-05 0,00E+00 2,91E-05 1,29E-04 3,18E-06 -5,54E-04
EP-terrestial mol N eq. 1,25E-02 2,26E-03 1,39E-02 4,60E-04 0,00E+00 3,21E-04 1,42E-03 1,71E-05 -6,18E-03
kg NMVOC
POCP 5,34E-03 6,31E-04 3,96E-03 1,65E-04 0,00E+00 9,18E-05 4,45E-04 6,40E-06 -2,66E-03
eq.
ADP-M&M kg Sb eq. 7,20E-05 1,97E-06 1,45E-05 1,58E-06 0,00E+00 3,70E-07 1,69E-06 4,25E-09 -8,17E-06
ADP-fossil MJ 4,48E+01 1,23E+00 8,82E+00 9,97E-01 0,00E+00 2,19E-01 1,36E+00 1,29E-02 -2,39E+01
WDP m³ 8,81E-01 3,62E-03 3,22E-02 1,86E-02 0,00E+00 6,74E-04 2,77E-02 6,78E-05 -3,93E-01
GWP-total: Global Warming Potential; GWP-fossil: Global Warming Potential fossil fuels; GWP-biogenic:
Global Warming Potential biogenic; GWP-LULUC: Global Warming Potential land use and land use change;
ODP: Depletion potential of the stratospheric ozone layer; AP: Acidification potential, Accumulated
Exceedance; EP-freshwater: Eutrophication potential, fraction of nutrients reaching freshwater end
compartment; See “additional Norwegian requirements” for indicator given as PO4 eq. EP-marine:
Eutrophication potential, fraction of nutrients reaching freshwater end compartment; EP-terrestial:
Eutrophication potential, Accumulated Exceedance; POCP: Formation potential of tropospheric ozone; ADP-
M&M: Abiotic depletion potential for non-fossil resources (minerals and metals); ADP-fossil: Abiotic
depletion potential for fossil resources; WDP: Water deprivation potential, deprivation weighted water
counsumption
EPD for the best environmental decision 9
Additional environmental impact indicators
A5 – insta-
Indicator Unit A1-A3 A4 A5 - other C1 C2 C3 C4 D
llation
Disease
PM 6,71E-08 6,93E-09 5,87E-08 1,97E-09 0,00E+00 1,29E-09 7,04E-09 8,85E-11 -3,22E-08
incidence
IRP kBq U235 eq. 4,09E-02 5,36E-03 3,90E-02 1,25E-03 0,00E+00 9,59E-04 4,08E-03 5,98E-05 -1,67E-02
ETP-fw CTUe 1,53E+01 9,82E-01 7,12E+00 4,08E-01 0,00E+00 1,78E-01 1,72E+00 1,21E-02 -5,64E+00
HTP-c CTUh 9,03E-10 3,65E-11 2,62E-10 3,78E-11 0,00E+00 6,34E-12 1,85E-10 3,19E-13 -4,58E-10
HTP-nc CTUh 1,54E-08 1,15E-09 8,43E-09 4,69E-10 0,00E+00 2,12E-10 2,34E-09 7,28E-12 -5,73E-09
SQP Dimensionless 8,29E+01 9,91E-01 7,31E+00 1,73E+00 0,00E+00 1,88E-01 1,08E+00 3,30E-02 -6,61E+01
PM: Particulate matter emissions; IRP: Ionising radiation, human health; ETP-fw: Ecotoxicity (freshwater);
ETP-c: Human toxicity, cancer effects; HTP-nc: Human toxicity, non-cancer effects; SQP: Land use related
impacts / soil quality
Classification of disclaimers to the declaration of core and additional environmental
impact indicators
ILCD
Indicator Disclaimer
classification
Global warming potential (GWP) None
ILCD type / level
Depletion potential of the stratospheric ozone layer (ODP) None
1
Potential incidence of disease due to PM emissions (PM) None
Acidification potential, Accumulated Exceedance (AP) None
Eutrophication potential, Fraction of nutrients reaching freshwater end
None
compartment (EP-freshwater)
Eutrophication potential, Fraction of nutrients reaching marine end
None
ILCD type / level compartment (EP-marine)
2
Eutrophication potential, Accumulated Exceedance (EP-terrestrial) None
Formation potential of tropospheric ozone (POCP) None
Potential Human exposure efficiency relative to U235 (IRP) 1
Abiotic depletion potential for non-fossil resources (ADP-minerals&metals) 2
Abiotic depletion potential for fossil resources (ADP-fossil) 2
Water (user) deprivation potential, deprivation-weighted water consumption
(WDP)
2
ILCD type / level
Potential Comparative Toxic Unit for ecosystems (ETP-fw) 2
3
Potential Comparative Toxic Unit for humans (HTP-c) 2
Potential Comparative Toxic Unit for humans (HTP-nc) 2
Potential Soil quality index (SQP) 2
Disclaimer 1 – This impact category deals mainly with the eventual impact of low dose ionizing radiation on
human health of the nuclear fuel cycle. It does not consider effects due to
possible nuclear accidents, occupational exposure nor due to radioactive waste disposal in underground facilities.
Potential ionizing radiation from the soil, from radon and from some
construction materials is also not measured by this indicator.
Disclaimer 2 – The results of this environmental impact indicator shall be used with care as the uncertainties on
these results are high or as there is limited experienced with the indicator
EPD for the best environmental decision 10
Resource use
A5 – insta-
Parameter Unit A1-A3 A4 A5 - other C1 C2 C3 C4 D
llation
RPEE MJ 1,71E+01 1,69E-02 1,51E-01 3,46E-01 0,00E+00 3,15E-03 6,70E-02 5,05E-04 -9,91E+00
RPEM MJ 0,00E+00 0,00E+00 0,00E+00 0,00E+00 0,00E+00 0,00E+00 0,00E+00 0,00E+00 0,00E+00
TPE MJ 1,71E+01 1,69E-02 1,51E-01 3,46E-01 0,00E+00 3,15E-03 6,70E-02 5,05E-04 -9,91E+00
NRPE MJ 4,80E+01 1,30E+00 9,36E+00 1,07E+00 0,00E+00 2,33E-01 1,45E+00 1,37E-02 -2,58E+01
NRPM MJ 0,00E+00 0,00E+00 0,00E+00 0,00E+00 0,00E+00 0,00E+00 0,00E+00 0,00E+00 0,00E+00
TRPE MJ 4,80E+01 1,30E+00 9,36E+00 1,07E+00 0,00E+00 2,33E-01 1,45E+00 1,37E-02 -2,58E+01
SM kg 0,00E+00 0,00E+00 0,00E+00 0,00E+00 0,00E+00 0,00E+00 0,00E+00 0,00E+00 0,00E+00
RSF MJ 0,00E+00 0,00E+00 0,00E+00 0,00E+00 0,00E+00 0,00E+00 0,00E+00 0,00E+00 0,00E+00
NRSF MJ 0,00E+00 0,00E+00 0,00E+00 0,00E+00 0,00E+00 0,00E+00 0,00E+00 0,00E+00 0,00E+00
W m3 1,51E-02 1,34E-04 4,99E-03 3,58E-04 0,00E+00 2,48E-05 9,33E-04 1,59E-05 -6,45E-03
RPEE Renewable primary energy resources used as energy carrier; RPEM Renewable primary energy
resources used as raw materials; TPE Total use of renewable primary energy resources; NRPE Non
renewable primary energy resources used as energy carrier; NRPM Non renewable primary energy
resources used as materials; TRPE Total use of non renewable primary energy resources; SM Use of
secondary materials; RSF Use of renewable secondary fuels; NRSF Use of non renewable secondary fuels; W
Use of net fresh water
End of life - Waste
A5 - A5 -
Parameter Unit A1-A3 A4 C1 C2 C3 C4 D
installation other
HW KG 1,49E-05 3,00E-06 2,26E-05 5,16E-07 0,00E+00 5,61E-07 2,28E-06 1,55E-08 -1,16E-05
NHW KG 1,31E-01 7,11E-02 5,13E-01 9,56E-03 0,00E+00 1,36E-02 6,86E-02 5,66E-02 -5,32E-02
RW KG 4,48E-05 8,36E-06 6,01E-05 1,49E-06 0,00E+00 1,49E-06 5,17E-06 8,41E-08 -1,73E-05
HW Hazardous waste disposed; NHW Non hazardous waste disposed; RW Radioactive waste disposed
End of life – output flow
A5 insta-
Parameter Unit A1-A3 A4 A5 - other C1 C2 C3 C4 D
llation
CR kg 0,00E+00 0,00E+00 1,51E-01 0,00E+00 0,00E+00 0,00E+00 0,00E+00 0,00E+00 0,00E+00
MR kg 0,00E+00 0,00E+00 5,30E-02 0,00E+00 0,00E+00 0,00E+00 4,62E-01 0,00E+00 0,00E+00
MER kg 0,00E+00 0,00E+00 1,24E-01 0,00E+00 0,00E+00 0,00E+00 1,80E-01 0,00E+00 0,00E+00
EEE MJ 0,00E+00 0,00E+00 0,00E+00 0,00E+00 0,00E+00 0,00E+00 0,00E+00 0,00E+00 5,48E+00
ETE MJ 0,00E+00 0,00E+00 0,00E+00 0,00E+00 0,00E+00 0,00E+00 0,00E+00 0,00E+00 8,30E-01
CR Components for reuse; MR Materials for recycling; MER Materials for energy recovery; EEE Exported
electric energy; ETE Exported thermal energy
Information describing the biogenic carbon content at the factory gate
Biogenic carbon content Unit Value
Biogenic carbon content in product kg C 0
Biogenic carbon content in the accompanying packaging kg C 0,41
EPD for the best environmental decision 11
Additional Norwegian requirements
Greenhous gas emission from the use of electricity in the manufacturing phase
National production mix from import, low voltage (production of transmission lines, in addition
to direct emissions and losses in grid) of applied electricity for the manufacturing prosess(A3).
National electricity grid Unit Value
Wind electricity, average (Ecoinvent 3.6) kg CO2 -eq/kWh 0,0263
Additional environmental impact indicators required in NPCR Part A for construction
products
In order to increase the transparency of biogenic carbon contribution to climate impact, the
indicator for GWP has been sub-divided into the following:
GWP-IOBC Climate impacts calculated according to the principle of instantanious oxidation
GWP-BC Climate impacts from the net uptake and emission of biogenic carbon from each
module.
A5 -
Indicator Unit A1-A3 A4 A5 – other C1 C2 C3 C4 D
installation
kg CO2
GWP-IOBC 1,43E+00 8,11E-02 5,77E-01 5,28E-02 0,00E+00 1,43E-02 5,23E-01 6,97E-03 -8,52E-01
eq.
kg CO2
GWP-BC -9,51E-01 4,38E-05 4,70E-04 9,56E-01 0,00E+00 8,68E-06 -5,42E-04 6,14E-06 -7,44E-04
eq.
kg CO2
GWP 4,77E-01 8,11E-02 5,78E-01 1,01E+00 0,00E+00 1,43E-02 5,22E-01 6,97E-03 -8,53E-01
eq.
GWP-IOBC Global warming potential calculated according to the principle of instantanious oxidation. GWP-
BC Global warming potential from net uptake and emissions of biogenic carbon from the materials in each
module. GWP Global warming potential
Hazardous substances
The declaration is based upon reference to threshold values and/or test results and/or material
safety data sheets provided to EPD verifiers. Documentation available upon request to EPD
owner.
✓ The product contains no substances given by the REACH Candidate list or the
Norwegian priority list.
□ The product contains substances given by the REACH Candidate list or the Norwegian
priority list that are less than 0,1 % by weight.
□ The product contain dangerous substances, more then 0,1% by weight, given by the
REACH Candidate List or the Norwegian Priority list, see table.
□ The product contains no substances given by the REACH Candidate list or the
Norwegian priority list. The product is classified as hazardous waste (Avfallsforskiften,
Annex III), see table.
Indoor environment
The product meets the requirements for low emissions.
Carbon footprint
Carbon footprint has not been worked out for the product.
EPD for the best environmental decision 12
Bibliography
ISO 14025:2010 Environmental labels and declarations - Type III environmental
declarations - Principles and procedures
ISO 14044:2006 Environmental management - Life cycle assessment -
Requirements and guidelines
EN 15804:2012+A2:2019 Sustainability of construction works - Environmental product
declaration - Core rules for the product category of construction
products
ISO 21930:2007 Sustainability in building construction – Environmental
declaration of building products
NPCR Part A Construction products and services. Ver. 2.0. March 2021, EPD-
Norge
CEWEP Results of Specific Data for Energy, R1 Plant Efficiency Factor and
NCV of 314 European Waste-to-Energy (WtE) Plants, CEWEP
Energy Report III (status 2007-2010), 2012, Reiman, D.O.
Program Operator tlf +47 23 08 80 00
The Norwegian EPD Foundation
Post Box 5250 Majorstuen, 0303 Oslo e-post: post@epd-norge.no
Norway web www.epd-norge.no
Publisher tlf +47 23 08 80 00
The Norwegian EPD Foundation
Post Box 5250 Majorstuen, 0303 Oslo e-post: post@epd-norge.no
Norway web www.epd-norge.no
Owner of the declaration tlf +4745190625
Norsk Wavin AS Fax
Karihaugveien 89, 1086, Oslo e-post: Invoice.no@wavin.com
Norway web www.wavin.com/nn-no
Author of the life cycle assessment tlf +31 (0)20 303 5777
Lisa Overmars Fax
H.J.E. Wenckebachweg 123, 1096 AM
e-post: lovermars@ecochain.com
Amsterdam
The Netherlands web www.ecochain.com
EPD for the best environmental decision 13
EPD for the best
environmental
decision
The Norwegian EPD foundation
www.epd-norge.no
