ENVIRONMENTAL PRODUCT DECLARATION
as per ISO 14025 and EN 15804+A2
Owner of the Declaration Kingspan Insulation B.V.
Publisher Institut Bauen und Umwelt e.V. (IBU)
Programme holder Institut Bauen und Umwelt e.V. (IBU)
Declaration number EPD-KIN-20230172-CBA1-EN
Issue date 11/07/2023
Valid to 10/07/2028
Therma™ TR29 / Therma™ TT49
Kingspan Insulation B.V.
www.ibu-epd.com | https://epd-online.com
General Information
Kingspan Insulation B.V. Therma™ TR29 / Therma™ TT49
Programme holder Owner of the declaration
IBU – Institut Bauen und Umwelt e.V. Kingspan Insulation B.V.
Hegelplatz 1 Lingewei 8
10117 Berlin 4004LL Tiel
Germany Netherlands
Declaration number Declared product / declared unit
EPD-KIN-20230172-CBA1-EN Therma™ TR29 / Therma™ TT49
1m2, 120mm thickness, R = 4,25 m2.K/W
D
This declaration is based on the product category rules: Scope:
Insulating materials made of foam plastics, 01/08/2021 The insulation materials Therma™ TR29 and Therma™ TT49 are
(PCR checked and approved by the SVR) produced by Kingspan Insulation at the manufacturing facility in Turnhout
(Belgium).
Therma™ TR29 Roof Board is a rigid thermoset polyisocyanurate (PIR)
Issue date fibre-free insulation board. Therma™ TR29 Roof Board is used as thermal
insulation under mechanically fixed or non-fixed ballasted roofing systems
11/07/2023
and can be used for (green) roofs where a high compressive strength is
required.
Therma™ TT49 Tapered Roof Board is a rigid thermoset PIR fibre-free
Valid to
insulation board. Therma™ TT49 Tapered Roof Board is used as thermal
10/07/2028 insulation under mechanically fixed or non-fixed ballasted roofing systems
and can be used for (green) roofs where a high compressive strength is
required. The product enhances water drainage from flat roofs.
In order to enable the user of the EPD to calculate the LCA results for
different thicknesses, the EPD contains the respective calculation rules.
The owner of the declaration shall be liable for the underlying information
and evidence; the IBU shall not be liable with respect to manufacturer
information, life cycle assessment data and evidences.
The EPD was created according to the specifications of EN 15804+A2. In
the following, the standard will be simplified as EN 15804.
Verification
Dipl.-Ing. Hans Peters
(Chairman of Institut Bauen und Umwelt e.V.) The standard EN 15804 serves as the core PCR
Independent verification of the declaration and data according to ISO
14025:2011
internally X externally
Florian Pronold Vito D'Incognito,
(Managing Director Institut Bauen und Umwelt e.V.) (Independent verifier)
1 Environmental Product Declaration - Kingspan Insulation B.V. - Therma™ TR29 / Therma™ TT49
Product
Performance data of the product in accordance with the
Product description/Product definition declaration of performance with respect to its essential
Therma™ TR29 Roof Board and Therma™ TT49 Tapered Roof characteristics according to EN 13165 - Thermal insulation
Board are rigid thermoset polyisocyanurate (PIR) fibre-free products for buildings - Factory made rigid polyurethane foam
insulation boards. The products are available in variable (PU) products - Specification.
thicknesses from 20 mm up to 200 mm. This EPD is based on a The declaration of performance of the product can be found at
thickness of 120 mm and R D-value of 4,25 m²·K/W. www.kingspan.com.
Base materials/Ancillary materials
For the placing on the market of the product in the European
Union/European Free Trade Association (EU/EFTA) (with the The product contains approximately 7,2 kg/m2 polyurethane
exception of Switzerland) Regulation (EU) No. 305/2011 (CPR) rigid foam.
applies. The product needs a declaration of performance taking The main materials of the polyurethane foam are MDI (between
into consideration EN 13165 - Thermal insulation products for 57-62 %), polyol (between 27-32 %) and a blowing agent
buildings - Factory made polyurethane foam (PU) products - (between 5-6 %). Due to the closed-cell structure (conform EN
specification and the CE-marking. For the application and use 13165), the blowing agent remains in the foam. Water, flame
the respective national provisions apply. retardants and additives are added (between 4-8 %).
In the current REACH regulations, polyurethane foam insulation
Application products are considered 'articles' and are exempt from the
Therma™ TR29 Roof Board is used as thermal insulation under requirements of Articles 57 and 59(1) of REACH Regulation
mechanically fixed or non-fixed ballasted roofing systems and (EC) No 1907/2006. These products are not classified as
can be used for (green) roofs where a high compressive 'hazardous products' according to any current legislation, and
strength is required. can hence be declared as follows:
- This article contains substances listed in the candidate list
Therma™ TT49 Tapered Roof Board is used as thermal (date: 31.08.2022) exceeding 0.1 percentage by mass: no.
insulation under mechanically fixed or non-fixed ballasted - This article contains other carcinogenic, mutagenic, reprotoxic
roofing systems and can be used for (green) roofs where a high (CMR) substances in categories 1A or 1B which are not on the
compressive strength is required. The product enhances water candidate list, exceeding 0.1 percentage by mass: no.
drainage from flat roofs. - Biocide products were added to this construction product or it
has been treated with biocide products (this then concerns a
Technical Data
treated product as defined by the (EU) Biocidal Products
Constructional data Regulation No. 528/2012
(BPR): no.
Name Value Unit
Thermal conductivity according to EN Reference service life
0.030 W/(m.K)
13165 for dN < 80mm The reference service life is not to be declared in this EPD as it
Thermal conductivity according to EN does not cover the use stage.
0.029 W/(m.K)
13165 for dN 80 - 119mm
Thermal conductivity according to EN
0.028 W(m.K)
13165 for dN ≥ 120mm
Reaction to fire according to EN 13165 E
Compressive strength according to EN CS(10\Y)
13165 400
Tensile strength according to EN 13165 TR200
Thickness tolerance according to EN
T3
13165
LCA: Calculation rules
The EPD is studied for a common product thickness of 120
Declared Unit mm. Multiplication factors are included to calculate impacts for
The declared unit (1 m²) and conversion factors are listed in the other product thicknesses within the range of 20 to 200 mm.
table below.
Declared unit
System boundary
Name Value Unit
The type of EPD according to EN 15804 is:
Declared unit 1 m2 cradle to gate with options, modules C1–C4, and
Gross density 60 kg/m3 module D (A1–A3, C, D and additional modules:
A4, A5).
Grammage 7.2 kg/m2
Layer thickness 0.12 m The product stage is a mandatory information module and it
The scope of this EPD is the thermal insulation product covers:
Therma™ TR29 / Therma™ TT49 as produced by Kingspan · A1, raw material extraction and processing, processing of
Insulation at the manufacturing facility in Turnhout (Belgium). secondary material input (e.g. recycling processes),
The environmental impacts have been calculated over the · A2, transport to the manufacturer,
calendar year 2021. · A3, manufacturing, including provision of all materials,
products and energy, packaging processing and its transport,
2 Environmental Product Declaration - Kingspan Insulation B.V. - Therma™ TR29 / Therma™ TT49
as well as waste processing up to the end-of-waste state or product at the end-of-life stage are assigned to the product
disposal of final residues system (C3); resulting potential credits for thermal and electrical
during the product stage. energy from energy substitution are declared in module D.
The construction process stage includes: Geographic Representativeness
· A4 transport to the building site; Land or region, in which the declared product system is
· A5 installation in the building including provision of all manufactured, used or handled at the end of the product´s
materials, products and energy, as well as waste processing up lifespan: Europe
to the end-of-waste state or disposal of final residues during the
construction process stage.
Comparability
Basically, a comparison or an evaluation of EPD data is only
The end-of-life stage is a mandatory information module and it
possible if all the data sets to be compared were created
covers:
according to EN 15804 and the building context, respectively
· C1 de-construction, demolition;
the product-specific characteristics of performance, are taken
· C2 transport to waste processing;
into account.
· C3 waste processing for reuse, recovery and/or recycling;
· C4 disposal (not applicable for this EPD) including provision
Background database
and all transport, provision of all materials, products and related
Background data from GaBi ts Version 10 is used with GaBi
energy and water use.
data sets CUP2022.1.
Environmental burden of the incineration (R1 > 60 %) of the
LCA: Scenarios and additional technical information
Characteristic product properties of biogenic carbon
The total mass of biogenic carbon containing materials is less
than 5 % of the total mass of the product and accompanying
Installation into the building (A5)
packaging.
Name ValueUnit
Technical information Total output substances following waste treatment
0.305 kg
The following technical information is a basis for the declared on site packaging material
modules or can be used for developing specific scenarios in the
The recycling of the packaging is considered in A5.
context of a building assessment.
End of life (C1-C4)
Manufacturing (A3)
A polyethylene packaging foil is used. The products are The assumptions for C1 are: diesel driven excavator (100 kW;
transported on wooden pallets. 0.2 litre fuel per ton excavated material). The assumptions for
Within Module A3 the following packaging of the final product is C2 are: Truck Euro 6, diesel driven, 26-28 t gross weight,
included: assumed distance 50 km
- Polyethylene cover and wrap: 0,010 kg/m² - Wooden pallet: Name Value Unit
0,295 kg/m² Collected as mixed construction waste 7.2 kg
Transport to the building site (A4) Energy recovery 7.2 kg
Name Value Unit
Reuse, recovery and/or recycling potentials (D), relevant
Litres of fuel 0.0103 l/100km scenario information
Transport distance 100 km Waste incineration with energy recuperation is assumed as
Gross density of products transported 60 kg/m3 end-of-life scenario
3 Environmental Product Declaration - Kingspan Insulation B.V. - Therma™ TR29 / Therma™ TT49
LCA: Results
DESCRIPTION OF THE SYSTEM BOUNDARY (X = INCLUDED IN LCA; ND = MODULE OR INDICATOR NOT DECLARED; MNR =
MODULE NOT RELEVANT)
Benefits and
Construction loads beyond
Product stage Use stage End-of-life stage
process stage the system
boundaries
la ire ta m w a Ry lp p u s tro p s n a rT g n iru tc a fu n a M e h t m o rf tro p s n a rTe tis e h t o t e ta g y lb m e s s A e s U e c n a n e tn ia M ria p e R tn e m e c a lp e R tn e m h s ib ru fe R y g re n e la n o ita re p Oe s u re ta w la n o ita re p Oe s u n o itc u rts n o c -e Dn o itilo m e d tro p s n a rT g n is s e c o rp e ts a W la s o p s iD -e s u e R-y re v o c e R-g n ilc y c e Rla itn e to p
A1 A2 A3 A4 A5 B1 B2 B3 B4 B5 B6 B7 C1 C2 C3 C4 D
X X X X X MND MND MNR MNR MNR MND MND X X X X X
RESULTS OF THE LCA - ENVIRONMENTAL IMPACT according to EN 15804+A2: 1m2 120mm Therma™ TR29 / Therma™ TT49
Parameter Unit A1-A3 A4 A5 C1 C2 C3 C4 D
GWP-total kg CO 2 eq 2.2E+01 6.03E-02 5.61E-01 4.6E-03 3.02E-02 1.59E+01 0 -6.31E+00
GWP-fossil kg CO 2 eq 2.24E+01 6.01E-02 3.26E-02 4.59E-03 3E-02 1.59E+01 0 -6.27E+00
GWP-biogenic kg CO 2 eq -4.7E-01 -8.3E-05 5.29E-01 6.15E-06 -4.15E-05 1.08E-03 0 -3.21E-02
GWP-luluc kg CO 2 eq 1.02E-02 3.35E-04 1.31E-06 5.67E-08 1.68E-04 2.82E-05 0 -6.91E-04
ODP kg CFC11 eq 5.14E-11 3.6E-15 4.45E-14 2.82E-16 1.8E-15 1.16E-12 0 -4.25E-11
AP mol H+ eq 4.18E-02 6.19E-05 7.86E-05 2.13E-05 3.1E-05 9.37E-03 0 -8.26E-03
EP-freshwater kg P eq 7.46E-05 1.79E-07 1.07E-08 9.26E-10 8.97E-08 3.13E-07 0 -8.65E-06
EP-marine kg N eq 1.15E-02 2.03E-05 2.55E-05 1.02E-05 1.01E-05 4.54E-03 0 -2.24E-03
EP-terrestrial mol N eq 1.18E-01 2.41E-04 3.74E-04 1.11E-04 1.21E-04 5.22E-02 0 -2.4E-02
kg NMVOC
POCP 5.33E-02 5.46E-05 6.95E-05 2.88E-05 2.73E-05 1.17E-02 0 -6.27E-03
eq
ADPE kg Sb eq 2.65E-05 5.02E-09 1.09E-09 1.88E-10 2.51E-09 3.2E-08 0 -9.48E-07
ADPF MJ 5.67E+02 8.03E-01 1.2E-01 6.21E-02 4.02E-01 4.1E+00 0 -1.07E+02
m3 world eq
WDP 2.7E+00 5.39E-04 5.77E-02 8.53E-06 2.7E-04 1.57E+00 0 -6.7E-01
deprived
GWP = Global warming potential; ODP = Depletion potential of the stratospheric ozone layer; AP = Acidification potential of land and water; EP =
Eutrophication potential; POCP = Formation potential of tropospheric ozone photochemical oxidants; ADPE = Abiotic depletion potential for non-fossil
resources; ADPF = Abiotic depletion potential for fossil resources; WDP = Water (user) deprivation potential)
RESULTS OF THE LCA - INDICATORS TO DESCRIBE RESOURCE USE according to EN 15804+A2: 1m2 120mm Therma™
TR29 / Therma™ TT49
Parameter Unit A1-A3 A4 A5 C1 C2 C3 C4 D
PERE MJ 4.4E+01 4.57E-02 4.45E+00 2.35E-04 2.28E-02 7.14E-01 0 -2.94E+01
PERM MJ 4.43E+00 0 -4.43E+00 0 0 0 0 0
PERT MJ 4.84E+01 4.57E-02 2.8E-02 2.35E-04 2.28E-02 7.14E-01 0 -2.94E+01
PENRE MJ 3.46E+02 8.05E-01 5.5E-01 6.23E-02 4.02E-01 2.25E+02 0 -1.07E+02
PENRM MJ 2.21E+02 0 -4.3E-01 0 0 -2.21E+02 0 0
PENRT MJ 5.68E+02 8.05E-01 1.2E-01 6.23E-02 4.02E-01 4.1E+00 0 -1.07E+02
SM kg 0 0 0 0 0 0 0 0
RSF MJ 0 0 0 0 0 0 0 0
NRSF MJ 0 0 0 0 0 0 0 0
FW m3 1.35E-01 5.16E-05 1.36E-03 3.54E-07 2.58E-05 3.68E-02 0 -2.82E-02
PERE = Use of renewable primary energy excluding renewable primary energy resources used as raw materials; PERM = Use of renewable primary
energy resources used as raw materials; PERT = Total use of renewable primary energy resources; PENRE = Use of non-renewable primary energy
excluding non-renewable primary energy resources used as raw materials; PENRM = Use of non-renewable primary energy resources used as raw
materials; PENRT = Total use of non-renewable primary energy resources; SM = Use of secondary material; RSF = Use of renewable secondary fuels;
NRSF = Use of non-renewable secondary fuels; FW = Use of net fresh water
RESULTS OF THE LCA – WASTE CATEGORIES AND OUTPUT FLOWS according to EN 15804+A2:
1m2 120mm Therma™ TR29 / Therma™ TT49
Parameter Unit A1-A3 A4 A5 C1 C2 C3 C4 D
HWD kg 1.82E-07 3.85E-12 1.15E-11 2.06E-13 1.93E-12 5.65E-10 0 -1.44E-08
NHWD kg 5.42E-01 1.15E-04 6.08E-03 5.83E-06 5.77E-05 8E-02 0 -5.4E-02
RWD kg 9.82E-03 9.91E-07 6.93E-06 6.82E-08 4.96E-07 1.69E-04 0 -8.42E-03
CRU kg 0 0 0 0 0 0 0 0
MFR kg 0 0 0 0 0 0 0 0
MER kg 0 0 3.05E-01 0 0 7.2E+00 0 0
EEE MJ 0 0 8.17E-01 0 0 2.75E+01 0 0
EET MJ 0 0 1.47E+00 0 0 4.91E+01 0 0
4 Environmental Product Declaration - Kingspan Insulation B.V. - Therma™ TR29 / Therma™ TT49
HWD = Hazardous waste disposed; NHWD = Non-hazardous waste disposed; RWD = Radioactive waste disposed; CRU = Components for re-use;
MFR = Materials for recycling; MER = Materials for energy recovery; EEE = Exported electrical energy; EET = Exported thermal energy
RESULTS OF THE LCA – additional impact categories according to EN 15804+A2-optional:
1m2 120mm Therma™ TR29 / Therma™ TT49
Parameter Unit A1-A3 A4 A5 C1 C2 C3 C4 D
Disease
PM 4.02E-07 3.57E-10 4.09E-10 2.42E-10 1.79E-10 2.6E-08 0 -6.85E-08
incidence
IR kBq U235 eq 1.06E+00 1.45E-04 1.13E-03 9.93E-06 7.26E-05 2.71E-02 0 -1.43E+00
ETP-fw CTUe 2.26E+02 5.58E-01 5.54E-02 4.33E-02 2.79E-01 1.4E+00 0 -2.35E+01
HTP-c CTUh 2E-08 1.12E-11 3.69E-12 8E-13 5.62E-12 1.06E-10 0 -1.08E-09
HTP-nc CTUh 1.93E-06 5.83E-10 1.54E-10 4.04E-11 2.92E-10 3.84E-09 0 -4.14E-08
SQP SQP 1.52E+02 2.76E-01 3.51E-02 1.71E-04 1.38E-01 8.58E-01 0 -1.91E+01
PM = Potential incidence of disease due to PM emissions; IR = Potential Human exposure efficiency relative to U235; ETP-fw = Potential comparative
Toxic Unit for ecosystems; HTP-c = Potential comparative Toxic Unit for humans (cancerogenic); HTP-nc = Potential comparative Toxic Unit for humans
(not cancerogenic); SQP = Potential soil quality index
Disclaimer 1 – for the indicator 'Potential Human exposure efficiency relative to U235'.This impact category deals mainly with the
eventual impact of low-dose ionizing radiation on human health of the nuclear fuel cycle. It does not consider effects due to possible
nuclear accidents, occupational exposure or to radioactive waste disposal in underground facilities. Potential ionizing radiation from the
soil, radon and from some construction materials is also not measured by this indicator.
Disclaimer 2 – for the indicators 'abiotic depletion potential for non-fossil resources', 'abiotic depletion potential for fossil resources',
'water (user) deprivation potential, deprivation-weighted water consumption', 'potential comparative toxic unit for ecosystems', 'potential
comparative toxic unit for humans – cancerogenic', 'Potential comparative toxic unit for humans - not cancerogenic', 'potential soil
quality index'. The results of this environmental impact indicator shall be used with care as the uncertainties on these results are high
as there is limited experience with the indicator.
Factors for different thicknesses
The LCA results for the insulation material declared in this EPD refer to a product with a thickness of 120 mm. To enable the user of the
EPD to calculate the results for different thicknesses the factors in the following table can be used for the calculation. The LCA results
in chapter 5 have to be multiplied with these factors.
This EPD was created using a software tool.
References
Biocidal Products Regulation No. 528/2012 (BPR) Specification
Regulation (EU) No 528/2012 of the European Parliament and
of the Council of 22 May 2012 concerning the making available EN 15804
on the market and use of biocidal products EN 15804:2012+A2:2019+AC:2021, Sustainability of
construction works — Environmental Product Declarations —
CPR Core rules for the product category of construction products.
Regulation (EU) No. 305/2011 of the European Parliament and
of the Council of 9 March 2011 laying down harmonised GaBi ts
condition for the marketing of construction products and thinkstep AG: Leinfelden-Echterdingen GaBi Software- System
repealing Council Directive 89/106/EC and Database for Life Cycle Engineering 1992- 2019
ISO 14025 IBU 2022
EN ISO 14025:2011, Environmental labels and declarations — Institut Bauen und Umwelt e.V.: General Instructions for the
Type III environmental declarations — Principles and EPD programme of Institut Bauen und Umwelt e.V., Version
procedures. 2.1, Berlin: Institut Bauen und Umwelt e.V., 2022. www.ibu-
epd.com
EN 13165
EN 13165:2012+A2:2016: Thermal insulation products for LCA-tool
buildings. Factory made polyurethane foam (PU) products. Kingspan LCA tool, version 1.1. IBU-KSI-202001-LT1- EN.
5 Environmental Product Declaration - Kingspan Insulation B.V. - Therma™ TR29 / Therma™ TT49
Developed by Sphera Solutions GmbH (formely Thinkstep Environmental Product Declarations of Institut Bauen und
GmbH) Umwelt (IBU), Part B: Requirements on the EPD for insulating
materials made of foam plastics. May 2023
PCR Version 1.7, Part A
Institut Bauen und Umwelt e.V., Berlin (pub.): Product Category REACH
Rules for Building-Related Products and services, Part A: Regulation (EC) No 1907/2006 of the European Parliament and
Calculation Rules for the Life Cycle Assessment and of the Council on the Registration, Evaluation, Authorisation
Requirements on the Project Report according to EN and Restriction of Chemicals (REACH)
15804+A2:2019 November 2021 https://echa.europa.eu/candidate-list-table;
PCR 2023, Part B Candidate list
Institut Bauen und Umwelt e.V., Berlin (pub.): Product Category https://echa.europa.eu/candidate-list-table; accessed
Rules for Construction Products from the range of 31.08.2022, 233 substances listed.
6 Environmental Product Declaration - Kingspan Insulation B.V. - Therma™ TR29 / Therma™ TT49
Publisher
Institut Bauen und Umwelt e.V. +49 (0)30 3087748- 0
Hegelplatz 1 info@ibu-epd.com
10117 Berlin www.ibu-epd.com
Germany
Programme holder
Institut Bauen und Umwelt e.V. +49 (0)30 3087748- 0
Hegelplatz 1 info@ibu-epd.com
10117 Berlin www.ibu-epd.com
Germany
Author of the Life Cycle Assessment
Kingspan Insulation B.V. +31 (0) 543 543 210
Lingewei 8 info@kingspaninsulation.nl
4004LL Tiel www.kingspan.com
Netherlands
Owner of the Declaration
Kingspan Insulation B.V. +31 (0) 543 543 210
Lingewei 8 info@kingspaninsulation.nl
4004LL Tiel www.kingspan.com
Netherlands
7 Environmental Product Declaration - Kingspan Insulation B.V. - Therma™ TR29 / Therma™ TT49
