ENVIRONMENTAL PRODUCT DECLARATION
as per ISO 14025 and EN 15804+A2
Owner of the Declaration Ideal standard International
Publisher Institut Bauen und Umwelt e.V. (IBU)
Programme holder Institut Bauen und Umwelt e.V. (IBU)
Declaration number EPD-IDE-20230198-IBB1-EN
Issue date 20.09.2023
Valid to 19.09.2028
Dual control and thermostatic fittings
Ideal Standard International
www.ibu-epd.com | https://epd-online.com
1. General Information
Ideal Standard International Dual control and thermostatic fittings
Programme holder Owner of the declaration
IBU – Institut Bauen und Umwelt e.V. Ideal standard International
Hegelplatz 1 Da Vincilaan 2
10117 Berlin 1935 Zaventem Belgium
Germany France
Declaration number Declared product / declared unit
EPD-IDE-20230198-IBB1-EN 1 kg of Dual control thermostatic fitting
This declaration is based on the product category rules: Scope:
Fittings and showers, 01.08.2021 The EPD covers a range of Dual control and thermostatic fittings,
(PCR checked and approved by the SVR) produced by Ideal Standard in two production plants, respectively in
Bulgaria and Germany.
Issue date The EPD includes the result of 1 kg of a representative product. The
representative product is a product produced in Bulgaria and has an
20.09.2023
absolute weight that is closest to the average weight of all fittings. Note
that in the EPD the LCI and LCA are converted to 1 kg of fitting. The
representativeness of the selected product and an estimation of the
Valid to
variability has been calculated in the LCA background report.
19.09.2028
Foreground data has been provided directly by Ideal Standard and
background LCA data is based on Ecoinvent 3.8 and Industry 2.0 data.
The owner of the declaration shall be liable for the underlying information
and evidence; the IBU shall not be liable with respect to manufacturer
information, life cycle assessment data and evidences.
The EPD was created according to the specifications of EN 15804+A2. In
the following, the standard will be simplified as EN 15804.
Verification
The standard EN 15804 serves as the core PCR
Dipl.-Ing. Hans Peters
Independent verification of the declaration and data according to ISO
(Chairman of Institut Bauen und Umwelt e.V.)
14025:2011
internally X externally
Florian Pronold Vito D'Incognito,
(Managing Director Institut Bauen und Umwelt e.V.) (Independent verifier)
1 Environmental Product Declaration - Ideal Standard International - Dual control and thermostatic fittings
2. Product
exceeding 0.1 percentage by mass,
2.1 Product description/Product definition
Thermostatic and Dual control fittings are a mechanical wall Biocide products were not added to this construction product
mounted fitting with hot and cold-water control. It includes many and it has not been treated with biocide products as defined by
components: cartridge, handles, flexhose, connectors, spout, the (EU) Ordinance on Biocide Products No. 528/2012.
… The range of thermostatic and dual control covers several
models and two commercial brands: Ideal Standard and 2.6 Manufacture
Porcher. Production brass components:
During the brass production Ideal Standard remelts internal
Thermostatic: Fittings that keep the water at a pre-determined, scrap with some purchased metals (eg. Al, Cu ...) to adjust for
fixed temperature, with one handle to control the water flow and the recipe. Besides, Ideal Standard also purchases brass rods
pressure. Most commonly a shower mixer, but if a dual control and tubes from their suppliers. The brass ingots from remelted
or single lever basin mixer has a thermostatic function, this scrap and the purchased brass rods and tubes are cutted,
should be classed as thermostatic. shaved and/or turned to produce the different brass
components. Finally the brass components are plated with
Dual Control: a two-handled mixer fitting. nickel and chrome. Also note that Ideal Standard sometimes
purchases completely finalized brass components if the
No DOP and CE marking is available. demand is higher than the produced quantity.
2.2 Application Production plastic components:
Solution used in private and public bathrooms. Basin mixer is a Some plastic components are produced at Ideal Standard.
plumbing fixture used to wash hands in lavatories and Plastic granulates are injection moulded into the correct shape.
bathrooms by mixing hot and cold water. Afterwards they are plated with nickel and chrome.
2.3 Technical Data
Assembly
Constructional data The final stage in the production process is the assembly of the
different brass components, plastic components and purchased
Name Value Unit
components (i.e screws, cartridges etc …), and the packaging.
Maximum load temperature permanent operation 65 °C
Maximum load temperature temporary operation 90 °C 2.7 Environment and health during manufacturing
Flow rate (indications for pressure range of 1-3 0.6 - Environmental, occupational health, safety and quality
m3/h
bar) 1.2 management at the Ideal Standard plants are in accordance
Sound emissions 20 dB with the following standards:
• ISO 14001
No DOP and CE marking is available.
• ISO 9001
2.4 Delivery status • ISO 45001
The products are packed with a PE plastic bag, a coverage
2.8 Product processing/Installation
carton and are accompanied with an instruction and guarantee
Usually, the fitting is installed using an installation kit provided
sheet.
by Ideal Standard (i.e. EasyKit), but it can also be installed
The products can come in very different shapes and
without.
dimensions. An overview of all Dual control thermostatic fittings
can be found on Ideal Standard's website and filter on 'Dual
2.9 Packaging
control' and 'Thermostatic':
PE plastic bag and coverage carton are used to pack and
https://www.idealstandard.co.uk/products/catalog/taps-and-
transport the product to the supplier/customer. The product is
mixers/basin-mixer-taps
also accompanied with an instruction and guarantee sheet.
2.5 Base materials/Ancillary materials
2.10 Condition of use
The main components of the product are: aerator, body, cap,
The product will not change in material composition over the
cartridge, flexhose, fixation screws, fixation set, handle, lift rod,
reference service life.
manifold and pop-up waste.
2.11 Environment and health during use
The material composition of the representative product:
Under normal conditions of use, the product do not cause any
• 95% Brass adverse health effects or release of volatile organic compounds
• 4% stainless steel (VOCs) into indoor air.
• 1% Plastic
The composition of all products included in the scope varies No environmental impact on water, air or soil is expected.
between:
2.12 Reference service life
• 75-99% Brass
Reference service life not relevant, as module B has not been
• 1-5% stainless steel
declared.
• 1-25% Plastic
This product does contain substances listed in the candidate 2.13 Extraordinary effects
list (date: 26.10.2022) exceeding 0.1 percentage by mass:
Fire
7439-92-1 (Pb)
Not subjected to fire classification.
This product does not contain other CMR substances in
Water
categories 1A or 1B which are not on the candidate list,
2 Environmental Product Declaration - Ideal Standard International - Dual control and thermostatic fittings
No risks are expected to occur in terms of environment and
human health. 2.15 Disposal
According to the average European end-of-life scenario
Mechanical destruction described in Annex C of the Product Environmental Footprint
In case of mechanical destruction, no risks are expected to Pilots (PEFCR) 6.3 guidance (version March 2018), the
occur in terms of environment and human health. following disposal scenarios have been considered: 5% of the
brass and other metals parts are landfilled, 45% of the plastic
2.14 Re-use phase parts are incinerated and 55% of the plastic parts are landfilled.
Recycling of the brass components is possible, and considered
in this LCA study using the average European end-of-life 2.16 Further information
scenario described in Annex C of the Product Environmental Additional information on Dual control thermostatic fitting
Footprint Pilots (PEFCR) 6.3 guidance, version March 2018. produced by Ideal Standard can be found at:
https://www.idealstandard.co.uk/products/catalog/taps-and-
Energy recovery of incineration of the plastic components is mixers/basin-mixer-taps
also considered in this study.
3. LCA: Calculation rules
for 'Climate change – biogenic', but this indicator only
3.1 Declared Unit contributes <1% to 'Cllimate change – total'. As a result we can
Declared unit consider the production in Bulgaria is representative for both
production plants.
Name Value Unit
Declared unit 1 kg
Different product compositions
Raw density (brass) 8890 kg/m³ Secondly the variance in composition of the different dual
control and thermostatic fittings is investigated. Note that Ideal
Standards produces approximately 500 different SKUs (Stock
This study reports the environmental impact of 1 kg of the
keeping units), so it would not be feasible to model each SKU
representative Dual control and thermostatic fitting.
separately. Therefore, one has decided to estimate the variance
by comparing the representative product with the dual control
The representative product has been defined as follows:
and thermostatic with the lowest weight and the highest weight.
• Calculate the average weight based on the weight and
For both the single score and most important impact indicators
sold quantities of the product in 2021. A Dual control
the reference product has a higher impact than the other two
thermostatic fitting produced by Ideal Standard weighs
products of the sample, respectively the highest and lowest
between approximately 0,69 to 6,06 kg excluding
weighted product. The maximal variance over all impact
packaging
indicators is +10% for 'Ionising radiation', and -34% for
• Select the product that has a weight closest to the
'Ecotoxicity freshwater'.
average weight.
• Convert the data for the selected Dual control
Besides, some other assumptions have been made:
thermostatic fitting to 1 kg
• For production waste only most relevant production
• Using this approach the selected representative product
waste streams have been considered (waste of ancillary
is product 'B7547AA' and is produced in Bulgaria.
materials and smaller waste flows have been excluded).
• Only most relevant ancillary materials have been
The representativeness of this product and an estimation of the
selected based on consumption rate andimportance in
variability has been studied in the LCA background report.
the production process.
• No data was available on the specific packaging per
The environmental impact of a specific Dual control and
rawmaterial/component. Therefore the packaging of the
thermostatic fitting can be calculated by multiplying the results
raw materials have been calculated based on the
of 1 kg of the representative Dual control thermostatic fitting
packaging waste reported in the factory.
with the respective weight of the product.
3.4 Cut-off criteria
3.2 System boundary
The following processes are excluded because data was not
Cradle-to-gate with options, including module A4-A5, C1-C4
available:
and D
• Transport of packaging raw materials
3.3 Estimates and assumptions
• Packaging and transport of ancillary materials used
The data used in this study is based on the composition of a during the production process
representative dual control and thermostatic fitting produced in • Packaging and transport of ancillary materials used
Bulgaria (i.e. BG51). In the LCA background report the during installation
representativeness is checked and the variability is estimated No further approximations have been made to replace the
for the total production of dual control and thermostatics missing data, as they were considered to be not relevant based
produced in Europe by Ideal Standard. on the first iterations of the results
Different production plants The following processes are considered below cut-off:
First the difference between the Bulgarian (i.e. BG51) and the
• For production waste only most relevant production
German (i.e. GE11) plant was investigated. For both the single
waste streams have been considered (waste of ancillary
score and most important impact indicators according to the
materials and smaller waste flows have been excluded).
PEF single score (climate change, resource use metals and
• Only most relevant ancillary materials have been
ecotoxicity freshwater) the variance is less than 3% over the
selected based on consumption rate and importance in
total life cycle (modules A1-C4). The maximal variance is 44%,
the production process.
3 Environmental Product Declaration - Ideal Standard International - Dual control and thermostatic fittings
• Environmental impacts caused by the personnel of the
production plants are not included in the LCA, e.g. 3.9 Allocation
waste from the cafeteria and sanitary installations, Allocation of secondary materials or secondary fuels is not
accidental pollution caused by human mistakes, or applicable for this study.
environmental effects caused by commuter traffic.
Heating or cooling of the plants in order to ensure a At Ideal Standards, different products are produced. Only
comfortable indoor climate for the personnel for facility level data were available for some inputs/outputs. The
example is also neglected. facility level data have been allocated based on the produced
mass.
3.5 Background data
• Amounts of the raw materials/components (module
Ecoinvent 3.8 and Industry 2.0
A1and A2) and the packaging of the final product have
been extracted from the bill of material. No allocation
3.6 Data quality
was necessary.
Foreground data is specific to Ideal Standard and is collected
• The data for the production process (module A3) i.e
for the reference year 2021. Background data is based on
input and outputs such as energy consumption, water
Ecoinvent 3.8 which is released in September 2021, and
consumption, production waste, ancillary materials and
Industry 2.0.
emissions are based on factory averages (total amount
in the factory converted to 1 kg based on the total
In the LCA background report the representativeness of the
production volume in kg).
reference product is checked and the variability is estimated for
• No data was available on the specific packaging per raw
the total production of dual control and thermostatics produced
material/component (module A1). Therefore the
in Europe by Ideal Standard. For more information see section
packaging of the raw materials have been calculated
3.3.
based on the packaging waste reported in the factory,
3.7 Period under review and allocated to 1 kg of product based on the total
production volume.
The data collected by Ideal Standard is based on data from the
production year 2021 for Dual control thermostatic fittings.
3.10 Comparability
3.8 Geographic Representativeness Basically, a comparison or an evaluation of EPD data is only
possible if all the data sets to be compared were created
Land or region, in which the declared product system is
according to EN 15804 and the building context, respectively
manufactured, used or handled at the end of the product´s
the product-specific characteristics of performance, are taken
lifespan: Europe
into account. Ecoinvent 3.8 and Industry 2.0
4. LCA: Scenarios and additional technical information
Name ValueUnit
Characteristic product properties of biogenic carbon
Packaging waste (paper and cardboard) PEF EOL
The product does not contain biogenic carbon, but its
scenario Europe for coverage carton packaging: 11 0.469 kg
accompanying packaging contains 0.21 kg C per kg of product
% incineration; 75 % recycling; 14 % landfill
in the form of paper and cardboard.
Packaging waste (PE) PEF EOL scenario Europe
Information on describing the biogenic carbon content at for PE packaging: 32 % incineration; 29 % 0.002 kg
factory gate recycling; 39 % landfill
Name ValueUnit
End of life (C1-C4)
kg
Biogenic carbon content in product - C According to the European average PEF scenario, 95% of the
brass, steel and zamak are recycled and 5 % is landfilled. The
Biogenic carbon content in accompanying kg
0.15 European average PEF scenario for plastics describes 45 %
packaging C
incineration and 55 % landfill.
Note: 1 kg biogenic Carbon is equivalent to 44/12 kg of CO2
Name Value Unit
Collected as mixed construction waste 1 kg
Reuse - kg
Recycling 0.91 kg
Transport to the building site (A4)
Energy recovery 0.02 kg
Name Value Unit
Landfilling 0.07 kg
Litres of fuel 260 l/100km
Transport distance 2000 km Reuse, recovery and/or recycling potentials (D), relevant
Capacity utilisation (including Default value scenario information
%
empty runs) Ecoinvent Module D contains the benefits and loads of recycling Brass
Gross density of products and steel parts, and the benefits of energy recovery during the
Not calculated kg/m3
transported incineration of the plastics.
Default value
Capacity utilisation volume factor Ecoinvent - Note that according to EN15804+A2 the recycled content
amount of the brass (i.e. 54 %) has been taken into account in
Installation into the building (A5) module D by subtracting this from the amount of scrap that will
It is considered that there is no assembly waste, based on the be recycled at the end-of-life.
fact that the product is prefabricated and installed by hand.
Only the impact of packaging waste has been considered.
4 Environmental Product Declaration - Ideal Standard International - Dual control and thermostatic fittings
Name Value Unit
Loads recycling of brass: Impact of the 0.95*0.95-
production process of brass excluding the 0.95*0.54 = kg
production of raw materials 0.39
Loads recycling of steel: Impact of the
electric arc furnace production excluding 0.01 kg
the prodution of the raw materials
Benefits recycling of brass: Avoided 0.95*0.95-
production of brass using 100 % primary 0.95*0.54 = kg
materials 0.39
Benefits recycling of steel: Avoided
production of steel using 100 % primary 0.01 kg
materials
Benefits energy recovery during
incineration of plastics: 20 % avoided 0.15 MJ
production of Heat from natural gas
Benefits energy recovery during
incineration of plastics: 10 % avoided 0.08 MJ
production of European average grid mix
5 Environmental Product Declaration - Ideal Standard International - Dual control and thermostatic fittings
5. LCA: Results
DESCRIPTION OF THE SYSTEM BOUNDARY (X = INCLUDED IN LCA; MND = MODULE OR INDICATOR NOT DECLARED; MNR
= MODULE NOT RELEVANT)
Benefits and
Construction loads beyond
Product stage Use stage End of life stage
process stage the system
boundaries
la ire ta m w a Ry lp p u s tro p s n a rT g n iru tc a fu n a M e h t m o rf tro p s n a rTe tis e h t o t e ta g y lb m e s s A e s U e c n a n e tn ia M ria p e R tn e m e c a lp e R tn e m h s ib ru fe R y g re n e la n o ita re p Oe s u re ta w la n o ita re p Oe s u n o itc u rts n o c -e Dn o itilo m e d tro p s n a rT g n is s e c o rp e ts a W la s o p s iD -e s u e R-y re v o c e R-g n ilc y c e Rla itn e to p
A1 A2 A3 A4 A5 B1 B2 B3 B4 B5 B6 B7 C1 C2 C3 C4 D
X X X X X MND MND MNR MNR MNR MND MND X X X X X
RESULTS OF THE LCA - ENVIRONMENTAL IMPACT according to EN 15804+A2: 1 kg Dual control thermostatic fitting
Parameter Unit A1 A2 A3 A4 A5 C1 C2 C3 C4 D
GWP-total kg CO 2 eq 3.99E+00 9.89E-02 5.77E+00 4.81E-01 7.37E-01 0 3.08E-02 1.39E-03 4.46E-02 -3.21E+00
GWP-fossil kg CO 2 eq 3.95E+00 9.88E-02 6.46E+00 4.8E-01 1.8E-02 0 3.08E-02 1.38E-03 4.46E-02 -2.66E+00
GWP-
biogenic kg CO 2 eq 2.47E-02 3.54E-05 -6.92E-01 1.72E-04 7.19E-01 0 1.1E-05 7.46E-06 2.58E-06 -5.47E-01
GWP-luluc kg CO 2 eq 8.26E-03 3.95E-05 3.76E-03 1.92E-04 8.17E-06 0 1.23E-05 3.19E-06 1.41E-06 -6.13E-03
ODP kg CFC11 eq 2.29E-07 2.29E-08 5.26E-07 1.11E-07 3.7E-09 0 7.14E-09 7.14E-11 4.61E-10 -1.55E-07
AP mol H+ eq 2.77E-01 2.81E-04 3.53E-02 1.36E-03 7.04E-05 0 8.74E-05 7.89E-06 1.57E-05 -2.13E-01
EP-
kg P eq 9.24E-04 7.05E-07 9.36E-04 3.42E-06 2.08E-07 0 2.2E-07 1.45E-07 4.38E-08 -6.21E-04
freshwater
EP-marine kg N eq 1.15E-02 5.58E-05 5.07E-03 2.71E-04 2.03E-05 0 1.74E-05 1.05E-06 8.66E-06 -8.2E-03
EP-terrestrial mol N eq 1.63E-01 6.22E-04 5.2E-02 3.02E-03 2.26E-04 0 1.94E-04 1.21E-05 6.64E-05 -1.16E-01
kg NMVOC
POCP 4.8E-02 2.39E-04 1.53E-02 1.16E-03 6.95E-05 0 7.44E-05 3.38E-06 1.8E-05 -3.53E-02
eq
ADPE kg Sb eq 4.06E-03 2.68E-07 9.89E-06 1.3E-06 4.67E-08 0 8.34E-08 7.81E-09 5.99E-09 -3.25E-03
ADPF MJ 5.28E+01 1.5E+00 1.17E+02 7.28E+00 2.42E-01 0 4.67E-01 2.88E-02 2.31E-02 -3.36E+01
m3 world eq
WDP 5.09E+00 4.56E-03 2.82E+00 2.22E-02 1.51E-03 0 1.42E-03 3.38E-04 8.59E-04 -4.06E+00
deprived
GWP = Global warming potential; ODP = Depletion potential of the stratospheric ozone layer; AP = Acidification potential of land and water; EP =
Eutrophication potential; POCP = Formation potential of tropospheric ozone photochemical oxidants; ADPE = Abiotic depletion potential for non-fossil
resources; ADPF = Abiotic depletion potential for fossil resources; WDP = Water (user) deprivation potential)
RESULTS OF THE LCA - INDICATORS TO DESCRIBE RESOURCE USE according to EN 15804+A2: 1 kg Dual control
thermostatic fitting
Parameter Unit A1 A2 A3 A4 A5 C1 C2 C3 C4 D
PERE MJ 5.68E-07 7.94E-09 1.94E-07 3.86E-08 1.39E-09 0 2.47E-09 2.63E-11 1.65E-10 -4.28E-07
PERM MJ 2.56E-01 6.5E-03 6.92E-01 3.16E-02 1.1E-03 0 2.03E-03 2.53E-04 1.07E-04 -1.63E-01
PERT MJ 1.83E+03 1.18E+00 4.2E+01 5.71E+00 3.11E-01 0 3.66E-01 1.91E-02 1.29E-01 -1.3E+03
PENRE MJ 5.65E-08 3.78E-11 2.02E-09 1.84E-10 2.47E-11 0 1.18E-11 9.63E-13 8.7E-12 -4.29E-08
PENRM MJ 4.01E-06 1.19E-09 8.76E-08 5.77E-09 2.98E-10 0 3.7E-10 1.88E-11 8.66E-11 -3.24E-06
PENRT MJ 9.11E+01 1.04E+00 4.95E+01 5.07E+00 1.75E-01 0 3.25E-01 1.89E-02 3.16E-02 -1.23E+02
SM kg 5.17E-01 0 2.32E-01 0 0 0 0 0 0 4.17E-01
RSF MJ 0 0 0 0 0 0 0 0 0 0
NRSF MJ 0 0 0 0 0 0 0 0 0 0
FW m3 1.14E-01 1.1E-04 5.16E-02 5.35E-04 7.5E-05 0 3.43E-05 2.15E-05 3.4E-05 -8.71E-02
PERE = Use of renewable primary energy excluding renewable primary energy resources used as raw materials; PERM = Use of renewable primary
energy resources used as raw materials; PERT = Total use of renewable primary energy resources; PENRE = Use of non-renewable primary energy
excluding non-renewable primary energy resources used as raw materials; PENRM = Use of non-renewable primary energy resources used as raw
materials; PENRT = Total use of non-renewable primary energy resources; SM = Use of secondary material; RSF = Use of renewable secondary fuels;
NRSF = Use of non-renewable secondary fuels; FW = Use of net fresh water
RESULTS OF THE LCA – WASTE CATEGORIES AND OUTPUT FLOWS according to EN 15804+A2:
1 kg Dual control thermostatic fitting
Parameter Unit A1 A2 A3 A4 A5 C1 C2 C3 C4 D
HWD kg 1.58E-03 3.91E-06 9.64E-03 1.9E-05 5.9E-07 0 1.22E-06 2.37E-08 5E-08 -1.08E-03
NHWD kg 1.58E+00 7.85E-02 1.15E+00 3.81E-01 7.79E-02 0 2.45E-02 1.12E-04 7.02E-02 -1.11E+00
RWD kg 1.9E-04 1.01E-05 6.14E-04 4.92E-05 1.6E-06 0 3.16E-06 2.1E-07 1.28E-07 -1.23E-04
CRU kg 0 0 0 0 0 0 0 0 0 0
MFR kg 0 0 5.62E-04 0 2.52E-01 0 0 9.15E-01 0 -1.17E+00
MER kg 0 0 0 0 0 0 0 0 0 0
EEE MJ 0 0 0 0 6.34E-02 0 0 0 5.44E-02 -1.18E-01
6 Environmental Product Declaration - Ideal Standard International - Dual control and thermostatic fittings
EET MJ 0 0 0 0 1.27E-01 0 0 0 1.09E-01 -2.36E-01
HWD = Hazardous waste disposed; NHWD = Non-hazardous waste disposed; RWD = Radioactive waste disposed; CRU = Components for re-use;
MFR = Materials for recycling; MER = Materials for energy recovery; EEE = Exported electrical energy; EET = Exported thermal energy
RESULTS OF THE LCA – additional impact categories according to EN 15804+A2-optional:
1 kg Dual control thermostatic fitting
Parameter Unit A1 A2 A3 A4 A5 C1 C2 C3 C4 D
Disease
PM 5.68E-07 7.94E-09 1.94E-07 3.86E-08 1.39E-09 0 2.47E-09 2.63E-11 1.65E-10 -4.28E-07
incidence
IR kBq U235 eq 2.56E-01 6.5E-03 6.92E-01 3.16E-02 1.1E-03 0 2.03E-03 2.53E-04 1.07E-04 -1.63E-01
ETP-fw CTUe 1.83E+03 1.18E+00 4.2E+01 5.71E+00 3.11E-01 0 3.66E-01 1.91E-02 1.29E-01 -1.3E+03
HTP-c CTUh 5.65E-08 3.78E-11 2.02E-09 1.84E-10 2.47E-11 0 1.18E-11 9.63E-13 8.7E-12 -4.29E-08
HTP-nc CTUh 4.01E-06 1.19E-09 8.76E-08 5.77E-09 2.98E-10 0 3.7E-10 1.88E-11 8.66E-11 -3.24E-06
SQP SQP 9.11E+01 1.04E+00 4.95E+01 5.07E+00 1.75E-01 0 3.25E-01 1.89E-02 3.16E-02 -1.23E+02
PM = Potential incidence of disease due to PM emissions; IR = Potential Human exposure efficiency relative to U235; ETP-fw = Potential comparative
Toxic Unit for ecosystems; HTP-c = Potential comparative Toxic Unit for humans (cancerogenic); HTP-nc = Potential comparative Toxic Unit for humans
(not cancerogenic); SQP = Potential soil quality index
Disclaimer 1 – for the indicator “Potential Human exposure efficiency relative to U235”. This impact category deals mainly with the
eventual impact of low-dose ionizing radiation on human health of the nuclear fuel cycle. It does not consider effects due to possible
nuclear accidents, occupational exposure or radioactive waste disposal in underground facilities. Potential ionizing radiation from the
soil, radon and from some construction materials is also not measured by this indicator.
Disclaimer 2 – for the indicators “abiotic depletion potential for non-fossil resources”, “abiotic depletion potential for fossil resources”,
“water (user) deprivation potential, deprivation-weighted water consumption”, “potential comparative toxic unit for ecosystems”,
“potential comparative toxic unit for humans – cancerogenic”, “Potential comparative toxic unit for humans - not cancerogenic”,
“potential soil quality index”. The results of this environmental impact indicator shall be used with care as the uncertainties on these
results are high as there is limited experience with the indicator.
6. LCA: Interpretation
The results show that for the Dual control thermostatic fitting, use – fossils’ the contribution of module A3 is more than 50 %.
the raw materials used in the formulation mix have a very
significant impact on all impact categories, due to the use of Outside the system’s boundaries, module D shows the benefits
brass. The brass has a dominant impact on 'Resource use – from recycling of the brass components and to a lesser extend
minerals and metals’ in particular. Besides the production of the the energy recovery from incineration of the plastic
raw materials, also module A3 (mainly energy consumption components. In module D the use of recycled content at the
during the manufacturing) has a significant contribution. For beginning of life has been taken into account in the
indicators such as ‘Global warming potential’ and ‘Resource calculations, as required by EN15804+A2.
7. Requisite evidence
8. References
Standards ISO 14025
EN ISO 14025:2011, Environmental labels and declarations —
EN15804 Type III environmental declarations — Principles and
EN 15804:2012+A2:2019+AC:2021, Sustainability of procedures.
construction works — Environmental Product Declarations —
Core rules for the product category of construction products. ISO 14040
ISO 14040:2006: Environmental management – Life cycle
PCR Part A assessment – Principles and framework.
Calculation rules for the Life Cycle Assessment and
Requirements on the Background Report, Institut Bauen und ISO 14044
Umwelt e.V., www.bauumwelt.com. IO 14044:2006: Environmental management – Life cycle
assessment – Requirements and guidelines.
PCR Part B
Institut Bauen und Umwelt e.V, Berlin (pub.): PCR Guidance- ISO 45001
Texts for Building-Related Products and Services From the ISO 45001:2018: Occupational health and safety management
range of Environmental Product Declarations of Institute systems Requirements with guidance for use
Construction and Environment e.V. (IBU) : Requirements on the
EPD Fittings and showers Further references
ISO 9001 Pré Consultants (2021)
ISO 9001:2015: Quality management systems — Requirements SimaPro 9.3.0.3 [Computer Software]. Amersfoort, The
Netherlands.
ISO 14001
ISO 14001:2015: Environmental management systems — CPR
Requirements with guidance for use European Regulation N° 305/2011 (CPR)
7 Environmental Product Declaration - Ideal Standard International - Dual control and thermostatic fittings
Ecoinvent
Wernet, G., Bauer, C., Steubing, B., Reinhard, J., Moreno-Ruiz, PEFCR
E., and Weidema, B., 2016. The ecoinvent database version 3 European commission (2018). Product Environmental Footprint
(part I): overview and methodology. The International Journal of Category Rules PEFCR Guidance, version 6.3.
Life Cycle Assessment, [online] 21(9), pp.1218–1230. Available
at: IBU
http://link.springer.com/10.1007/s11367-016-1087-8 IBU 2021. Institut Bauen und Umwelt e.V.: General Instructions
for the EPD programme of Institut Bauen und Umwelt e.V.,
Industry 2.0 Version 2.0, Berlin: Institut Bauen und Umwelt e.V., 2021
Industry 2.0 (from PlasticsEurope, worldsteel and ERASM) LCA www.ibu-epd.com
database as integrated in SimaPro 9.3.0.3.
8 Environmental Product Declaration - Ideal Standard International - Dual control and thermostatic fittings
Publisher
Institut Bauen und Umwelt e.V. +49 (0)30 3087748- 0
Hegelplatz 1 info@ibu-epd.com
10117 Berlin www.ibu-epd.com
Germany
Programme holder
Institut Bauen und Umwelt e.V. +49 (0)30 3087748- 0
Hegelplatz 1 info@ibu-epd.com
10117 Berlin www.ibu-epd.com
Germany
Author of the Life Cycle Assessment
Enperas +32 3 376 00 19
Thorpark 8300 info@enperas.com
3600 Genk https://www.enperas.com/en/
Belgium
Owner of the Declaration
Ideal standard International +33622608444
Da Vincilaan 2 eboukari@idealstandard.com
1935 Zaventem Belgium www.idealstandard.com
France
9 Environmental Product Declaration - Ideal Standard International - Dual control and thermostatic fittings
