ENVIRONMENTAL PRODUCT DECLARATION
as per ISO 14025 and EN 15804+A2
Owner of the Declaration Knauf Ceiling Solutions GmbH & Co. KG
Publisher Institut Bauen und Umwelt e.V. (IBU)
Programme holder Institut Bauen und Umwelt e.V. (IBU)
Declaration number EPD-KNA-20210115-IBD2-EN
Issue date 25.05.2021
Valid to 24.05.2026
AMF THERMATEX & ARMSTRONG Acoustic Range (Pontarlier)
Knauf Ceiling Solutions GmbH & Co. KG
www.ibu-epd.com | https://epd-online.com
1. General Information
Knauf Ceiling Solutions GmbH & Co. KG AMF THERMATEX & ARMSTRONG Acoustic
Range (Pontarlier)
Programme holder Owner of the declaration
IBU – Institut Bauen und Umwelt e.V. Knauf Ceiling Solutions GmbH & Co. KG
Hegelplatz 1 Elsenthal 15
10117 Berlin 94481 Grafenau
Germany Germany
Declaration number Declared product / declared unit
EPD-KNA-20210115-IBD2-EN 1 m² THERMATEX/ARMSTRONG Acoustic Range mineral ceiling tiles with
an average surface weight of 2,84 kg/m².
This declaration is based on the product category rules: Scope:
Mineral panels, 01.08.2021 This document refers to 1 m² THERMATEX/ARMSTRONG Acoustic Range
(PCR checked and approved by the SVR) mineral ceiling tiles with an average recipe and an average surface weight
of 2,84 kg/m², manufactured at the production facility in Pontarlier, France
under the brand names THERMATEX and ARMSTRONG.
Issue date The owner of the declaration shall be liable for the underlying information
and evidence; the IBU shall not be liable with respect to manufacturer
25.05.2021
information, life cycle assessment data and evidences.
The EPD was created according to the specifications of EN 15804+A2. In
Valid to
the following, the standard will be simplified as EN 15804.
24.05.2026
Verification
The standard EN 15804 serves as the core PCR
Independent verification of the declaration and data according to ISO
14025:2011
internally X externally
Dipl.-Ing. Hans Peters
(Chairman of Institut Bauen und Umwelt e.V.)
Florian Pronold Prof. Dr. Birgit Grahl,
(Managing Director Institut Bauen und Umwelt e.V.) (Independent verifier)
1 Environmental Product Declaration - Knauf Ceiling Solutions GmbH & Co. KG - AMF THERMATEX & ARMSTRONG Acoustic Range (Pontarlier)
2. Product
Name Value Unit
2.1 Product description/Product definition
Mineral wool 20 - 90 %
The ceiling tiles are manufactured using a wet felt process and
Perlite 8 - 35 %
consist of biosoluble mineral wool, perlite, clay and starch. The
ceiling tiles meet the requirements of DIN 18177 and EN Clay 0 - 25 %
13964. Cellulose fibres 2 - 5 %
Starch 5 - 15 %
The AMF and Armstrong mineral tiles are available in a wide
others 0 - 5 %
range of different surface designs and product properties.
Depending on the design, the ceiling tiles are available in In addition, glass fiber fleece and dispersion paints are used on
different formats and edge finishes. the surface and water for preparation during production. The
recycled content is at least 42 %.
This EPD applies to the following products:
Armstrong Perla OP 0.95, Armstrong Perla OP 1.00, Armstrong This product/article/at least one partial article contains
Ultima+ Alpha, THERMATEX Acoustic, Ultima+ Acoustic, substances listed in the ECHA-candidate list (date: 25.06.2020)
Armstrong Perla, Armstrong Bioguard Acoustic, Armstrong exceeding 0.1 percentage by mass: No
Bioguard Acoustic OP, Armstrong Saniguard, Armstrong Sierra,
Armstrong Sierra OP, Armstrong Solara, THERMATEX Antaris, This product/article/at least one partial article contains other
THERMATEX Antaris C. Armstrong Ultima, THERMATEX carcinogenic mutagenic reprotoxic (CMR) substances in
Thermofon, Adagio Acoustic+, Adagio Alpha+.The declared categories 1A or 1B which are not on the candidate list,
average represents a potential underestimation of the exceeding 0.1 percentage by mass: No
environmental impact associated to the products Perla OP1.
For the placing on the market of the product in the European Biocide products were added to this construction product or it
Union/European Free Trade Association (EU/EFTA) (with the has been treated with biocide products (this then concerns a
exception of Switzerland) Regulation (EU) No. 305/2011 (CPR) treated product as defined by the (EU) Ordinance on Biocide
applies. The product needs a declaration of performance taking Products No. 528/2012): No
into consideration EN 13964:2014, suspended ceiling
requirements and test methods and the CE-marking. For the In-can preservatives are used in the production process;
application and use the respective national provisions apply. however, they are not part of the products and are therefore not
within the scope of the Ordinance on Biocide Products.
2.2 Application
Mineral tiles (wet-felt) are typically used as lay in for suspended Colemanite (2CaO – 3B2O3 – 5H2O) is used as a flame
ceiling constructions. They are primarily used as optical retardant in some tiles up to 2 % in the final product.
cladding, but also for sound absorption and sound insulation,
for fire resistance and against fire spreading, for cleanrooms 2.6 Manufacture
and high hygiene requirements. The mineral tiles are produced in the traditional wet process
(wet-felt). The raw materials are mixed with water to form a
2.3 Technical Data homogeneous suspension, which is pumped onto a belt
Mineral boards (wet-felt) are regulated by EN 13964 and have conveyor (Fourdrinier). The water is removed mechanically
corresponding labelling and declaration of performance. The (gravity and vacuum) and by evaporation in the drying oven. As
following data provide an overview of results: far as possible, the process water is reused. It is treated
accordingly and fed back into the process water circuit.
Construction data (according to DIN 18177)
Depending on the desired appearance the panels can be
Name Value Unit
sanded, colour-treated, patterned, eroded or embossed.
0.04 - Production waste and dust are reused in the process in the
Thermal conductivity W/(mK)
0.06 sense of an internal cycle.
Sound absorption coefficient acc. ISO 354 The manufacturing plant is certified according to ISO 9001, ISO
0.65 - 1 %
and ISO 11654 14001 and OHSAS 18001.
Airborne sound reduction acc. ISO 10848-2
25 - 38 dB 2.7 Environment and health during manufacturing
and EN 717-1
The manufacturer complies with all European regulations for
150 -
Gross density kg/m3 the production of mineral slabs:
270
• The manufacturing plant is certified according to ISO
Performance data of the product in accordance with the
9001, ISO 14001 and OHSAS 18001
declaration of performance with respect to its essential
• The production has a closed water cycle, i.e. no waste
characteristics according to EN 13964:2014, suspended ceiling
water is produced
requirements and test methods (not part of CE-marking).
• Production generates virtually almost no waste, all
resulting blanks, dust and rejects are reused to 99%
2.4 Delivery status
• Exclusive use of mineral fibres according to Regulation
The EPD refers to panels with a thickness between 15 - 20 mm
(EU) No.1272/2008 Note Q
which can have variable length and width dimensions.
• Prohibition of the production and use of biopersistent
2.5 Base materials/Ancillary materials fibres (Ordinance on Hazardous Substances, Annex II,
No. 5)
Mineral tile composition:
• Prohibition of placing biopersistent fibres on the market
(Chemicals Prohibition Order, No.23 of the Annex to §1)
• Not subject to declaration according to REACH
2 Environmental Product Declaration - Knauf Ceiling Solutions GmbH & Co. KG - AMF THERMATEX & ARMSTRONG Acoustic Range (Pontarlier)
designation (and also many other European countries) with
2.8 Product processing/Installation negligible smoke development and no burning drip in the event
There are no recognised systemic hazards associated with the of fire.
installation of ceiling tiles. It is recommended that materials are
Fire Reaction
handled in a manner that minimises dust generation. Workers
should wear appropriate personal protective equipment. Name Value
Equipment such as gloves, goggles and dust masks are Building material class A2
recommended to minimise exposure to dust and prevent skin Smoke gas development s1
irritation.
Burning droplets d0
2.9 Packaging
The panels are packaged with cardboard boxes and sealed Water
with transparent polyethylene film.These packages lie on In the case of prolonged contact with water, the starch binder
chemically untreated wooden pallets. The pallets are wrapped dissolves, which can lead to a loss of structure, and if the
with polyethylene stretch film. Foil, paper and wood can be soluble components are discharged into the sewage treatment
recycled in the usual ways. plant, they are biodegradable, increasing the chemical oxygen
demand (COD) and the biological oxygen demand (BOD).
2.10 Condition of use
When handled properly, the mechanical and structural-physical Mechanical destruction
properties of the mineral tile remain intact throughout its entire The mineral tiles (wet-felt) can be broken by hand and also
service life. Direct contact with water should be avoided due to damaged superficially, which can result in dust formation.
the water-soluble binding agent starch.
2.14 Re-use phase
2.11 Environment and health during use If the panels are removed properly, they can be reinstalled. In
When properly installed, no dust/particles are released during case of minor damage, the slabs can be reused as cut-to-size
the use phase. For the substance groups formaldehyde, volatile tiles. Mineral tiles can be returned to the manufacturing process
organic compounds (VOCs) and total volatile organic if they are of the correct type and have sufficient material
compounds (TVOCs), the limits according to DIN 18177 are quality; they can be recycled up to 100 %.
complied with.
2.15 Disposal
2.12 Reference service life The waste code number of production residues for mineral tiles
The service life of the mineral tiles (wet-felted) is up to 50 according to the AVV, German List of Wastes Ordinance is 10
years, depending on the area of use, exposure and state of 11 03, the waste code number for construction site waste
maintenance. Within the framework of the conditions of use, no (offcuts) is 17 06 04. If the tiles are not recycled as described in
ageing effects are to be expected apart from visual 2.14., they are disposed of in a landfill.
discolouration caused by air circulation.
2.16 Further information
2.13 Extraordinary effects Further information at www.knaufceilingsolutions.com
Fire DoPs at knaufamf-dop.com or
The declared products are classified in the fire reaction class www.knaufarmstrong.com/dop.html
A2-s1, d0 according to EN 13501-1. This means that they are
"non-combustible" according to the German building authority
3. LCA: Calculation rules
products included in the average was considered.
3.1 Declared Unit
This EPD refers to a declared unit of 1 m² 3.2 System boundary
THERMATEX/Armstrong Acoustic Range ceiling tiles with an The life cycle assessment of average THERMATEX/Armstrong
average surface weight of 2,84 kg/m². Acoustic Range mineral ceiling tiles includes a cradle-to-gate
analysis of the products' environmental impacts with options.
Declared unit
Subsequent life cycle phases are part of the analysis:
Name Value Unit
Declared unit 1 m2 Module A1–A3 | Production stage
Grammage 2.84 kg/m2 The production stage includes the upstream burdens of raw
material supply, their transports and the manufacturing plant of
Layer thickness 0,017 m
Knauf Ceiling Solutions located in Pontarlier (France). Mineral
conversion factor [Mass/Declared Unit] 2.84 -
ceiling tiles are produced in the wet-felt process.
The ceiling tiles are produced at the Knauf Ceiling Solutions Main raw material inputs, therefore, refer to mineral wool,
production site in Pontarlier, France under the brand names perlite, clay and starch. The production site is supplied with
THERMATEX and Armstrong. electricity from the French power grid and thermal energy from
natural gas.
Various types of mineral ceiling tiles are produced at the site. A
differentiation between the product groups was made based on Module A4 | Transport from the gate to the site
the recipe of the products. Acoustic products have common Module A4 includes transport to the construction site. For this
product components and are manufactured in different purpose, transport by truck over a distance of 470 km is used
thicknesses. Acoustic panels are provided with a glass fleece as a representative scenario.
coating. The calculation of the weighted average recipe and
surface weight is based on the square meters produced of each Module A5 | Assembly at the site
product. Ensuring the correct representation of the average For installation in the building, a scenario of 5 % loss is
composition of the raw boards, the recipe of each of the declared in this EPD. The losses during installation in the
3 Environmental Product Declaration - Knauf Ceiling Solutions GmbH & Co. KG - AMF THERMATEX & ARMSTRONG Acoustic Range (Pontarlier)
building are strongly dependent on the building geometry and 10; 2020.2).
the specific application. Thus, the percentage of waste can vary
greatly in the building context and must be adjusted accordingly 3.6 Data quality
at the building level according to the actual conditions. In Data collection is based on product-specific questionnaires. It
addition to the losses during installation in the building, Module follows an iterative process clarifying questions via e-mail,
A5 includes the environmental impacts from the End-of-Life of telephone calls or in personal/web meetings. Intensive
the packaging of the products. discussions between Knauf Ceiling Solutions and Daxner &
Merl results in an accurate mapping of product-related material
Module C1 | Deconstruction and demolition and energy flows. This leads to a high quality of foreground
Disassembly of the product is done either manually or using data collected. Data collection relies on a consistent process
smaller tools. Referring energy demand is considered to be according to ISO 14044.
negligible.
The weighted average was calculated based on the product-
Modul C2 | Transport to disposal specific recipes and composition. Its representativity is
The transport to the disposal of the material is estimated considered to be good for 88 % of the THERMATEX/Armstrong
declaring a 50 km radius to the landfill. In reality, this scenario Acoustic products.
may vary depending on the actual location of deconstruction
and referring waste treatment. The technological, geographical and time-related
representativeness of the database was kept in mind when
Module C3 | Waste processing selecting background data. Whenever specific data were
The declared scenario assumes landfilling of the product. missing, either generic datasets or representative average data
Referring environmental impacts are accounted for in module were used instead. The implemented GaBi background
C4. datasets refer to the latest versions available (not more than
ten years old) and are carefully chosen.
Module C4 | Disposal
3.7 Period under review
Module C4 refers to the emissions from the disposal of the
mineral ceiling tiles. The chosen scenario, therefore, includes Foreground data were collected in the 2019 production year,
the environmental burdens of landfilling of the product. and the data are based on the volumes produced on an annual
basis.
Module D | Benefits and loads beyond the system
3.8 Geographic Representativeness
boundary
Land or region, in which the declared product system is
The declared scenario assumes landfilling of the product.
manufactured, used or handled at the end of the product´s
Referring environmental impacts are accounted for in module
lifespan: France
C4. Module D declares the substitution potential from energy
recovery of the incineration of packaging waste in module A5.
3.9 Allocation
3.3 Estimates and assumptions
All information for the allocation of given material and energy
Assumptions and approximations are applied in case of a lack
flows is based on the site-related evaluations. The calculation
of representative data. All assumptions and approximations are
of specific input quantities for the raw board production of the
documented precisely and represent a best-guess
analysed product group is based on the respective recipe. In
representation of reality. In case of uncertainty, a conservative
addition, product-specific application rates (e.g. basecoat, top
approach is chosen.
coat, glass fleece etc.) were available for the upscaling of
3.4 Cut-off criteria referring input quantities. Total annual energy consumption and
waste flows are allocated based on the production share of
The LCA model covers all available input and output flows,
each product.
which can be represented based on robust data. Data gaps are
filled with conservative assumptions from average data (when
For in the production used waste paper, the system boundary is
available) or with generic data and are documented
set after sorting. It is assumed that the end of waste status has
accordingly. Only data with a contribution lower 1 % were cut
been reached. Waste glass wool does not reach the end of
off. Thus, no data were neglected, of which a substantial impact
waste status. The system boundary for secondary raw
is to be expected. All relevant data were collected
materials defined in EN 15804 applies.
comprehensively. Cut-off material and energy flows were
chosen carefully based on their expected quantitative
3.10 Comparability
contribution as well as potential environmental impacts. Thus, it
Basically, a comparison or an evaluation of EPD data is only
can be assumed that the sum of all neglected input flows does
possible if all the data sets to be compared were created
not account for more than 5 % of the total material, water and
according to EN 15804 and the building context, respectively
energy flows.
the product-specific characteristics of performance, are taken
3.5 Background data into account. Zur Berechnung der Ökobilanz wurde die
-Hintergrunddatenbank verwendet
This study uses generic background data for the evaluation of
upstream environmental impacts from GaBi databases (GaBi
4. LCA: Scenarios and additional technical information
Name ValueUnit
Characteristic product properties of biogenic carbon
kg
The biogenic carbon content quantifies the amount of biogenic Biogenic carbon content in product 0.12
C
carbon in the declared product.
Biogenic carbon content in accompanying kg
Information on the description of the biogenic carbon packaging 0.06 C
content at the factory gate
4 Environmental Product Declaration - Knauf Ceiling Solutions GmbH & Co. KG - AMF THERMATEX & ARMSTRONG Acoustic Range (Pontarlier)
End-of-Life (C1-C4)
Name Value Unit
Collected separately 2.84 kg
Landfilling 2.84 kg
Transport to the site (A4)
Name Value Unit
Litres of fuel (fully loaded) 53 l/100km
Litres of fuel (empty) 14 l/100km
Transport distance 470 km
Capacity utilisation (including empty runs) 61 %
Gross density of products transported 173 kg/m3
Assembly (A5)
Name Value Unit
Packaging (cardboard) 0,02 kg/m²
Packaging (pallets) 0,12 kg/m²
Packaging (PE-foil) 0,01 kg/m²
Reference service life
Name Value Unit
Placing on the market according to
Declared product
EN 13964; see also document
properties (at the -
centre on the website
gate) and finishes
knaufceilingsolutions.com
Design application
parameters (if
instructed by the
manufacturer), See document centre on the
-
including the website knaufceilingsolutions.com
references to the
appropriate practices
and application codes
Indoor environment
The exposure classes of ceiling
(for indoor
tiles vary depending on the
applications), e.g.
product, from a fluctuating relative -
temperature,
humidity up to 95 % at 30 °C,
moisture, chemical
without corrosive impurities.
exposure
Usage conditions,
No mechanical stress during
e.g. frequency of use, -
conventional use.
mechanical exposure
As a rule, the ceiling tiles do not
Maintenance e.g.
need to be cleaned for the duration
required frequency,
of their use in normal application.
type and quality and -
However, the ceiling tiles can be
replacement of
cleaned dry and damp according to
components
the cleaning guideline.
5 Environmental Product Declaration - Knauf Ceiling Solutions GmbH & Co. KG - AMF THERMATEX & ARMSTRONG Acoustic Range (Pontarlier)
5. LCA: Results
The following table contains the LCA results for a declared unit of 1 m² average THERMATEX/Armstrong Acoustic Range mineral
ceiling tiles with an average surface weight of 2,84 kg/m².
DESCRIPTION OF THE SYSTEM BOUNDARY (X = INCLUDED IN LCA; ND = MODULE OR INDICATOR NOT DECLARED; MNR =
MODULE NOT RELEVANT)
Benefits and
Construction loads beyond
Product stage Use stage End of life stage
process stage the system
boundaries
la ire ta m w a Ry lp p u s tro p s n a rT g n iru tc a fu n a M e h t m o rf tro p s n a rTe tis e h t o t e ta g y lb m e s s A e s U e c n a n e tn ia M ria p e R tn e m e c a lp e R tn e m h s ib ru fe R y g re n e la n o ita re p Oe s u re ta w la n o ita re p Oe s u n o itc u rts n o c -e Dn o itilo m e d tro p s n a rT g n is s e c o rp e ts a W la s o p s iD -e s u e R-y re v o c e R-g n ilc y c e Rla itn e to p
A1 A2 A3 A4 A5 B1 B2 B3 B4 B5 B6 B7 C1 C2 C3 C4 D
X X X X X MND MND MNR MNR MNR MND MND X X X X X
RESULTS OF THE LCA - ENVIRONMENTAL IMPACT according to EN 15804+A2: 1 m² THERMATEX/Armstrong Acoustic Range
mineral ceiling tiles (2,84 kg/m²)
Parameter Unit A1-A3 A4 A5 C1 C2 C3 C4 D
GWP-total kg CO 2 eq 3.87E+00 7.96E-02 2.46E-01 0 8.47E-03 0 4.74E-01 -8.95E-03
GWP-fossil kg CO 2 eq 4.32E+00 8.06E-02 2.47E-01 0 8.58E-03 0 4.31E-02 -8.94E-03
GWP-biogenic kg CO 2 eq -4.49E-01 -1.98E-03 -8.78E-04 0 -2.1E-04 0 4.31E-01 -1.11E-06
GWP-luluc kg CO 2 eq 1.9E-03 9.6E-04 1.02E-04 0 1.02E-04 0 1.24E-04 -2.61E-06
ODP kg CFC11 eq 1.54E-11 1.3E-17 7.69E-13 0 1.38E-18 0 1.6E-16 -6.96E-17
AP mol H+ eq 1.79E-02 2.88E-04 9.15E-04 0 3.06E-05 0 3.09E-04 -8.35E-06
EP-freshwater kg P eq 7.8E-05 5.55E-07 3.9E-06 0 5.91E-08 0 7.4E-08 -5.66E-09
EP-marine kg N eq 3.39E-03 1.25E-04 1.74E-04 0 1.34E-05 0 7.95E-05 -3.01E-06
EP-terrestrial mol N eq 5.47E-02 1.43E-03 2.79E-03 0 1.53E-04 0 8.74E-04 -3.2E-05
kg NMVOC
POCP 7.61E-03 2.44E-04 3.95E-04 0 2.59E-05 0 2.41E-04 -8.59E-06
eq
ADPE kg Sb eq 5.21E-07 7.54E-09 2.63E-08 0 8.02E-10 0 3.87E-09 -1.23E-09
ADPF MJ 7.94E+01 1.04E+00 4E+00 0 1.11E-01 0 5.65E-01 -2.58E-01
m3 world eq
WDP 2.02E-01 1.19E-03 1.3E-02 0 1.26E-04 0 4.51E-03 -5.52E-04
deprived
GWP = Global warming potential; ODP = Depletion potential of the stratospheric ozone layer; AP = Acidification potential of land and water; EP =
Eutrophication potential; POCP = Formation potential of tropospheric ozone photochemical oxidants; ADPE = Abiotic depletion potential for non-fossil
resources; ADPF = Abiotic depletion potential for fossil resources; WDP = Water (user) deprivation potential)
RESULTS OF THE LCA - INDICATORS TO DESCRIBE RESOURCE USE according to EN 15804+A2: 1 m²
THERMATEX/Armstrong Acoustic Range mineral ceiling tiles (2,84 kg/m²)
Parameter Unit A1-A3 A4 A5 C1 C2 C3 C4 D
PERE MJ 4.23E+00 8.47E-02 2.16E-01 0 9.01E-03 0 7.4E-02 -2.67E-02
PERM MJ 5.58E+00 0 2.79E-01 0 0 0 0 0
PERT MJ 9.81E+00 8.47E-02 4.95E-01 0 9.01E-03 0 7.4E-02 -2.67E-02
PENRE MJ 7.87E+01 1.05E+00 3.97E+00 0 1.11E-01 0 5.65E-01 -2.58E-01
PENRM MJ 6.7E-01 0 3.35E-02 0 0 0 0 0
PENRT MJ 7.94E+01 1.05E+00 4E+00 0 1.11E-01 0 5.65E-01 -2.58E-01
SM kg 8.99E-01 0 4.49E-02 0 0 0 0 0
RSF MJ 0 0 0 0 0 0 0 0
NRSF MJ 0 0 0 0 0 0 0 0
FW m3 6.44E-03 1.36E-04 3.92E-04 0 1.44E-05 0 1.43E-04 -6.29E-05
PERE = Use of renewable primary energy excluding renewable primary energy resources used as raw materials; PERM = Use of renewable primary
energy resources used as raw materials; PERT = Total use of renewable primary energy resources; PENRE = Use of non-renewable primary energy
excluding non-renewable primary energy resources used as raw materials; PENRM = Use of non-renewable primary energy resources used as raw
materials; PENRT = Total use of non-renewable primary energy resources; SM = Use of secondary material; RSF = Use of renewable secondary fuels;
NRSF = Use of non-renewable secondary fuels; FW = Use of net fresh water
RESULTS OF THE LCA – WASTE CATEGORIES AND OUTPUT FLOWS according to EN 15804+A2:
1 m² THERMATEX/Armstrong Acoustic Range mineral ceiling tiles (2,84 kg/m²)
Parameter Unit A1-A3 A4 A5 C1 C2 C3 C4 D
HWD kg 4.17E-07 1.31E-07 2.13E-08 0 1.4E-08 0 8.62E-09 -5.92E-11
NHWD kg 6.54E-01 2.23E-04 1.75E-01 0 2.38E-05 0 2.84E+00 -7.23E-05
RWD kg 4.58E-03 5.06E-06 2.3E-04 0 5.38E-07 0 6.42E-06 -4.67E-05
CRU kg 0 0 0 0 0 0 0 0
MFR kg 0 0 0 0 0 0 0 0
MER kg 0 0 0 0 0 0 0 0
6 Environmental Product Declaration - Knauf Ceiling Solutions GmbH & Co. KG - AMF THERMATEX & ARMSTRONG Acoustic Range (Pontarlier)
EEE MJ 0 0 6.18E-02 0 0 0 0 0
EET MJ 0 0 1.1E-01 0 0 0 0 0
HWD = Hazardous waste disposed; NHWD = Non-hazardous waste disposed; RWD = Radioactive waste disposed; CRU = Components for re-use;
MFR = Materials for recycling; MER = Materials for energy recovery; EEE = Exported electrical energy; EET = Exported thermal energy
RESULTS OF THE LCA – additional impact categories according to EN 15804+A2-optional:
1 m² THERMATEX/Armstrong Acoustic Range mineral ceiling tiles (2,84 kg/m²)
Parameter Unit A1-A3 A4 A5 C1 C2 C3 C4 D
Disease
PM 1.58E-07 1.68E-09 8.1E-09 0 1.79E-10 0 3.83E-09 -7.07E-11
incidence
IR kBq U235 eq 1.09E+00 1.17E-03 5.44E-02 0 1.24E-04 0 6.6E-04 -1.19E-02
ETP-fw CTUe 2.39E+01 8.63E-01 1.21E+00 0 9.18E-02 0 3.23E-01 -6.86E-02
HTP-c CTUh 2.82E-09 1.93E-11 1.44E-10 0 2.06E-12 0 4.79E-11 -1.47E-12
HTP-nc CTUh 5.85E-08 1.25E-09 3.2E-09 0 1.33E-10 0 5.27E-09 -5.42E-11
SQP SQP 6.96E+01 7.39E-01 3.48E+00 0 7.86E-02 0 1.18E-01 -1.28E-02
PM = Potential incidence of disease due to PM emissions; IR = Potential Human exposure efficiency relative to U235; ETP-fw = Potential comparative
Toxic Unit for ecosystems; HTP-c = Potential comparative Toxic Unit for humans (cancerogenic); HTP-nc = Potential comparative Toxic Unit for humans
(not cancerogenic); SQP = Potential soil quality index
Disclaimer 1 – for the indicator “Potential Human exposure efficiency relative to U235”. This impact category deals mainly with the
eventual impact of low-dose ionizing radiation on human health of the nuclear fuel cycle. It does not consider effects due to possible
nuclear accidents, occupational exposure or radioactive waste disposal in underground facilities. Potential ionizing radiation from the
soil, radon and from some construction materials is also not measured by this indicator.
Disclaimer 2 – for the indicators “abiotic depletion potential for non-fossil resources”, “abiotic depletion potential for fossil resources”,
“water (user) deprivation potential, deprivation-weighted water consumption”, “potential comparative toxic unit for ecosystems”,
“potential comparative toxic unit for humans – cancerogenic”, “Potential comparative toxic unit for humans - not cancerogenic”,
“potential soil quality index”. The results of this environmental impact indicator shall be used with care as the uncertainties on these
results are high as there is limited experience with the indicator.
6. LCA: Interpretation
The following interpretation contains a summary of the LCA THERMATEX/Armstrong Acoustic Range mineral ceiling tiles.
results referenced to a functional unit of 1 m² average
Life of the products due to landfilling (module C4) have a minor
contribution.
The comparison of the product's life cycle phases shows a
clear dominance of the production phase (modules A1-A3) in all The direct emissions from the combustion of natural gas for the
environmental impact categories. The potential environmental production process represent the main driver when it comes to
impacts from transport to disposal (module C2) and the End-of- potential climate change (GWP) as well as depletion of fossil
7 Environmental Product Declaration - Knauf Ceiling Solutions GmbH & Co. KG - AMF THERMATEX & ARMSTRONG Acoustic Range (Pontarlier)
resources (ADPF). Potential acidification (AP), photooxidant
creation (POCP) as well as terrestrial eutrophication (EP- The declared environmental impacts represent a weighted
terrestrial) are dominated by direct emissions from natural gas average of the THERMATEX/Armstrong Acoustic product
combustion, the upstream supply chain of stone wool as well as group. The analysis of the variance of the specific composition
starch. Potential eutrophication of marine ecosystems (EP- of the products within the group shows a good representativity
marine) is mainly affected by upstream emission from starch of the results for 88 % of the production quantity (range of -6 %
production and direct emissions at the site as well. When it and +33 %).
comes to eutrophication potential of freshwater (EP-freshwater)
the share of the upstream supply chain of starch represents the The environmental impacts of Perla OP95 and Sierra Solara
most dominant factor. Electricity from the French grid products are potentially overrated. In contrast, THERMATEX
represents an important driver when it comes to potential water Perla OP1 products are potentially underrated (+30 to +70 %
scarcity (WDP). except for ODP).
7. Requisite evidence
7.1 Radioactivity
AgBB Overview (28 days)
Not applicable for these products.
Name Value Unit
7.2 Biopersistence TVOC (C6 - C16) 0,028 mg/m3
The mineral wool used for the production of the panels is TSVOC (C16 - C22) < 0,005 mg/m3
biosoluble and, according to EU Regulation 1272/2008/EC, is R (dimensionless) 0,0048
to be assessed as free of suspected cancer. "EUCEB"
VOC without NIK 0,021 mg/m3
organization monitors and guarantees the quality of the wool
Carcinogenic substances < 0,001 mg/m3
used.
The production and use of non-exempt fibres is prohibited by
the Ordinance on Hazardous Substances and the Chemicals 7.4 Formaldehyde
Prohibition Ordinance. Measuring point: Eurofins Product Testing A/S
Test report: VOC emission test report Indoor Air Comfort GOLD
7.3 VOC emissions (10.02.2021)
Measuring point: Eurofins Product Testing A/S Number: 392-2020-00519911_A_EN rev 1
Test report: VOC emission test report Indoor Air Comfort GOLD Testing period: 17.11.2020-11.02.2021
(10.02.2021) Test basis: EN 16516
Number: 392-2020-00519911_A_EN rev 1 The product complies with formaldehyde class E1 according to
Testing period: 17.11.2020-11.02.2021 EN 16516.
Test basis: ISO 16000-6, EN 16516
8. References
Standards absorption in reverberant rooms.
DIN 18177 ISO 717-1
DIN 18177:2012, Mineral tiles manufactured in the factory by DIN EN ISO 717-1:2013-06, Acoustics - Assessment of sound
the wet felt process - Characteristic values and test methods. insulation in buildings and of building elements - Part 1:
Airborne sound insulation.
EN 13501-1
DIN EN 13501-1:2019, Classification of construction products ISO 9001
and building elements according to their reaction to fire, Part 1: DIN EN ISO 9001:2015-11, Quality management systems -
Classification with the results of tests on the reaction to fire of Requirements.
construction products.
ISO 10848-2
EN 13964 DIN EN ISO 10848-2:2006-08, Acoustics - Measurement of
DIN EN 13964:2014, Suspended ceilings - Requirements and airborne and impact sound transmission between adjacent
test methods. rooms in test stands - Part 2: Application to lightweight
components where the connection has a minor influence.
EN 15804
DIN EN 15804:2012+A2:2019, Sustainability of construction ISO 11654
works - Environmental product declarations - Core rules for the DIN EN ISO 11654:1997-07, Acoustics - Sound absorbers for
product category of construction products. use in buildings - Evaluation of sound absorption.
EN 16487 ISO 14001
DIN EN 16487:2015-02, Acoustics - Test specifications for DIN EN ISO 14001:2015-11, Environmental management
suspended ceilings - Sound absorption. systems - Requirements with guidance for use.
EN 16516 ISO 14025
DIN EN 16516:2020-10, Construction products: Assessment of DIN EN ISO 14025:2011-10, Environmental labels and
release of dangerous substances - Determination of emissions declarations - Type III environmental declarations - Principles
into indoor air. and procedures.
ISO 354 ISO 14044
DIN EN ISO 354:2003-12, Acoustics - Measurement of sound DIN EN ISO 14044:2006-10, Environmental management – Life
8 Environmental Product Declaration - Knauf Ceiling Solutions GmbH & Co. KG - AMF THERMATEX & ARMSTRONG Acoustic Range (Pontarlier)
cycle assessment – Requirements and guidelines.
IBU 2016
ISO 16000-6 Institut Bauen und Umwelt e.V.: General Programme
ISO 16000-6:2011-12, Indoor air contaminants - Part 6: Instructions for the Preparation of EPDs at the Institut Bauen
Determination of VOCs in indoor air and test chambers, und Umwelt e.V. Version 1.1, Berlin: Institut Bauen und Umwelt
sampling on Tenax TA®, thermal desorption and gas e.V., 2016. www.ibu-epd.com.
chromatography with MS/FID.
Ordinance on Biocide Products
OHSAS 18001 Regulation (EU) No 528/2012 of the European Parliament and
OHSAS 18001-2007, Certification of occupational safety and of the Council of 22 May 2012 concerning the making available
health management systems. on the market and use of biocidal products.
Further References Ordinance on Hazardous Substances
Ordinance on Hazardous Substances, of 26 November 2010
AgBB (Federal Law Gazette I p. 1643, 1644), last amended by Article
Ausschuss zur gesundheitlichen Bewertung von Bauprodukte 148 of the Law of 29 March 2017 (Federal Law Gazette I p.
(AgBB) (Committee for health-related evaluation of building 626).
products): Vorgehensweise bei der gesundheitlichen
Bewertung der Emissionen von flüchtigen organischen PCR Part A
Verbindungen (VOC und SVOC) aus Bauprodukten. Institut Bauen und Umwelt e.V. (IBU), 2019. Product Category
Rules for Building-Related Products and Services. Part A:
AVV, German List of Wastes Ordinance Calculation Rules for the Life Cycle Assessment and
Regulation on the European Waste List. Requirements on the Project Report. Version 1.8.
Chemicals Prohibition Ordinance PCR: Mineral panels
Chemicals Prohibition Ordinance (German designation: Institut Bauen und Umwelt e.V. (IBU), 2019. Product Category
Chemikalien-Verbotsverordnung – ChemVerbotsV) of 20 Rules for Building-Related Products and Services. Part B:
January 2017 (Federal Law Gazette I p. 94; 2018 I p. 1389), Requirements on the EPD for Mineral panels. Version 1.1.
last amended by Article 300 of the Ordinance of 19 June 2020 10.12.2018.
(Federal Law Gazette I p. 1328).
REACH
ECHA-candidate list Regulation (EC) No 1907/2006 of the European Parliament and
List of substances of very high concern (SVHC) for Council from 18 December 2006, Regulation concerning the
authorisation (ECHA Candidate List), 25.06.2020, published Registration, Evaluation, Authorisation and Restriction of
under Article 59 (10) of REACH. Helsinki: European Chemicals Chemicals (REACH).
Agency.
Regulation (EU) Nr. 305/2011(CPR)
EUCEB Regulation (EU) No 305/2011 of the European Parliament and
EUCEB, European Certification Board for Mineral Wool of the Council of 9 March 2011 laying down harmonised
Products. Brussels, Belgium. conditions for the marketing of construction products and
repealing Council Directive 89/106/EEC Text with EEA
Eurofins Product Testing A/S relevance.
Test report: VOC emission test report Indoor Air Comfort GOLD
(10.02.2021), Number: 392-2020-00519911_A_EN rev 1. Regulation (EU) Nr.1272/2008
Regulation (EC) No 1272/2008 of the European Parliament and
GaBi of the Council of 16 December 2008 on classification, labelling
GaBi 10, Software-System and Database for Life Cycle and packaging of substances and mixtures, amending and
Engineering. DB v8.7 2020.2. Stuttgart, Echterdingen: Sphera, repealing Directives 67/548/EEC and 1999/45/EC, and
1992-2020. Available at: http://documentation.gabi- amending Regulation (EC) No 1907/2006.
software.com.
9 Environmental Product Declaration - Knauf Ceiling Solutions GmbH & Co. KG - AMF THERMATEX & ARMSTRONG Acoustic Range (Pontarlier)
Publisher
Institut Bauen und Umwelt e.V. +49 (0)30 3087748- 0
Hegelplatz 1 info@ibu-epd.com
10117 Berlin www.ibu-epd.com
Germany
Programme holder
Institut Bauen und Umwelt e.V. +49 (0)30 3087748- 0
Hegelplatz 1 info@ibu-epd.com
10117 Berlin www.ibu-epd.com
Germany
Author of the Life Cycle Assessment
Daxner & Merl GmbH +43 676 849477826
Lindengasse 39/8 office@daxner-merl.com
1070 Wien www.daxner-merl.com
Austria
Owner of the Declaration
Knauf Ceiling Solutions GmbH & Co. KG 0049 8552 422 0
Elsenthal 15 info@knaufamf.com
94481 Grafenau www.knaufceilingsolutions.com
Germany
10 Environmental Product Declaration - Knauf Ceiling Solutions GmbH & Co. KG - AMF THERMATEX & ARMSTRONG Acoustic Range (Pontarlier)
