ENVIRONMENTAL PRODUCT DECLARATION
as per ISO 14025 and EN 15804+A1
Owner of the Declaration Troldtekt A/S
Programme holder Institut Bauen und Umwelt e.V. (IBU)
Publisher Institut Bauen und Umwelt e.V. (IBU)
Declaration number EPD-TRO-20210190-IBA1-EN
Issue date 12.11.2021
Valid to 11.11.2026
Acoustic panels - painted
Troldtekt 35mm Natural Grey
www.ibu-epd.com | https://epd-online.com
Umwelt Produktdeklaration Name des Herstellers – Name des Produkts
1. General Information
Troldtekt A/S Troldtekt Natural Grey – painted
Programme holder Owner of the declaration
IBU – Institut Bauen und Umwelt e.V. Troldtekt A/S
Panoramastr. 1 Sletvej 2 A
10178 Berlin 8310 Tranbjerg
Germany Denmark
Declaration number Declared product / declared unit
EPD-TRO-20210190-IBA1-EN Acoustic panel "Natural Grey" - 1 m2, 35 mm thickness
- painted finish
This declaration is based on the product Scope:
category rules: This declaration represents the production, supply,
Wood cement - Mineral-bonded wooden composites, mounting, use, dismantling and disposal of 1 m2 (35
01.2019 mm thickness) of grey cement-bonded wood wool
(PCR checked and approved by the SVR) acoustic panel "Natural Grey" with a painted
finish, produced by Troldtekt A/S, with a reference
service life of 50 years. The production facility is
Issue date
located in Jutland, Denmark. Three scenarios
12.11.2021
represent its use in indoor conditions in Denmark,
Sweden and Germany.
Valid to
11.11.2026
The owner of the declaration shall be liable for the
underlying information and evidence; the IBU shall not
be liable with respect to manufacturer information, life
cycle assessment data and evidences.
The EPD was created according to the specifications
of EN 15804+A1. In the following, the standard will be
simplified as EN 15804.
Verification
The standard EN 15804 serves as the core PCR
Independent verification of the declaration and data
according to ISO 14025:2010
Dipl. Ing. Hans Peters internally x externally
(chairman of Institut Bauen und Umwelt e.V.)
Dr. Alexander Röder Ms Jane Anderson
(Managing Director Institut Bauen und Umwelt e.V.)) (Independent verifier)
2. Product
2.1 Product description/Product definition 2.2 Application
Troldtekt Natural Grey acoustic panels are some of the The panels are installed on the ceilings and walls in
leading and preferred solutions for creating a good offices, businesses, schools, institutions, cultural sites,
indoor sound environment. They are sold in various sports centers, swimming pools and private homes.
thicknesses (20-35 mm) and dimensions (width: 600
mm, lengths: 600/1200/2400 mm or width: 625 mm, 2.3 Technical Data
lengths: 625/1250/2500 mm). The panels can be The table below indicates the technical specifications
unpainted or painted in a wide variety of colors. of the panels in accordance with EN 13168, the
standard for cement-bonded wood wool and double-
For the placing on the market of the product in the layer panels with cement-bonded wood wool, and EN
European Union/European Free Trade Association 13964, the standard for suspended ceilings.
(EU/EFTA) (with the exception of Switzerland)
Regulation (EU) No. 305/2011 (CPR) applies. The
product needs a declaration of performance taking into
consideration EN 13964:2014, Suspended ceilings.
Requirements and test methods, and the CE-marking.
For the application and use, the respective national
provisions apply.
2 Environmental Product Declaration Troldtekt A/S – Troldtekt 35mm Natural Grey - painted
Technical specifications of the product covered in
this EPD 2.9 Packaging
Name Value Unit The product is packaged with plastic film and
Gross density 402 kg/m3 cardboard. The packaging material can be easily
Grammage 13,86 kg/m2 sorted and treated in dedicated waste recycling
Thermal conductivity acc. to DIN channels. The packaged product is delivered on a
76 W/(mK)
52612 returnable wood pallet.
Water vapour diffusion resistance
- -
factor acc. to DIN 4108-4
Sound absorption coefficient (only 2.10 Condition of use
with reference to the - % Conditions of use are detailed
corresponding component design) here: https://www.troldtekt.com/Installation/Use_and_
Light reflection (measured by maintenance
26,3 - 70,8 %
DELTA Light and Optics
Reaction to fire B/S1/d0 2.11 Environment and health during use
Environmental and ecotoxicity risks from exposure to
Troldtekt panel products during use have been
assessed and found eligible to the following
Performance data of the product in accordance with
certification schemes:
the declaration of performance with respect to its
essential characteristics according to EN  Finnish M1 classification
13168:2012+A1:2015, Thermal insulation products for  Danish Indoor Climate
buildings. Factory made wood wool (WW) products.  Blauer Engel
Specification, and EN 13964:2014, Suspended
 Cradle to Cradle
ceilings. Requirements and test methods.
2.4 Delivery status These certificates can be accessed
The panel is usually distributed in length of 600, 1200 here: https://www.troldtekt.com/Web-
or 2400 mm by 600 mm width or in length of 625, 1250 tools/Downloads/Certificates-and-tests
or 2500 mm by 625 mm width. It comes in three
thicknesses: 20, 25 and 35 mm. Additionally, several 2.12 Reference service life
density ranges are available: Coarse, Fine and Ultra- The technical service life of the panel is superior to 50
Fine causing different densities (388-428 kg/m3). The years. This EPD refers to the service lifetime indicated
panels are normally delivered in packs of 56 units on by the BBSR table for the material 353.311 of type
pallets. “Holzbekleidungen: Holz, Holzwerkstoff und
Mehrschichtleichtbauplatten”.
2.5 Base materials/Ancillary materials
The composition of the finished product is a mix of Because the panel is used in a building, in this EPD its
wood wool (29,1%), Portland cement (66,7%), water reference service life is limited by the expected service
(1,8%), as well as water glass (<1%) and accelerator life of the building, which is commonly accepted as 50
(<1%). Additionally, a painted finish is provided with a years, at least as LCA timeframe.
water-based paint (1,0%). The composition is at dry
basis at the factory gate, as most of the water has There is no influence of the ageing of the material on
evaporated during drying, but water remains bound to its technical performances.
the wood fibre and cement paste (hydrated cement).
2.13 Extraordinary effects
2.6 Manufacture
Norway spruce logs from local forests (with a moisture Fire
content of about 65-70%) are received and the bark is Information on the fire performance according to EN
removed. The wood is stored for approximately six 13168.
months until the moisture content in the wood drops to
29%. The wood is then shredded to produce wool. The Fire protection
wood wool is mixed together with Portland cement, Name Value
water, and additives. The mixture is cast and cured Building material class B
using a heat press and dried with a biomass-fired Burning droplets d0
oven. The cast panel is milled to remove any material Smoke gas development S1
in excess and cut edges. After approximately 4 weeks
of curing, the panel can be painted before being stored Water
on a pallet and packaged to be transported to central No information on the product performance under the
distribution warehouses. unforseeable influence of water is available.
2.7 Environment and health during Mechanical destruction
manufacturing No information on the product performance under
Troldtekt is following its working environment closely. unforseeable mechanical destruction is available.
Both the physical working environment and sickness
absence are closely monitored. It is an ongoing 2.14 Re-use phase
process involving both leaders and factory workers. Currently, Troldtekt panels undergo thermal treatment
with energy recovery. Composting is also possible.
2.8 Product processing/Installation
Installation instructions are available here: Additional information on recycling
https://www.troldtekt.com/Installation options: https://www.troldtekt.com/~/media/Files/Info%
3 Environmental Product Declaration Troldtekt A/S – Troldtekt 35mm Natural Grey - painted
20sheets/English/Troldtekt_Recycling%20instructions
%20pdf.pdf Additional information on disposal
options: https://www.troldtekt.com/environment-and-
2.15 Disposal csr/product-life-cycle/recycling/
The product may be composted, thermally treated with
energy recovery, or landfilled. 2.16 Further information
For additional information on technical specifications,
European Waste Code: 10 13 11 (wastes from you may consult the Declaration Of
cement-based composite materials) Performance: https://www.troldtekt.com/Web-
tools/Downloads/DoPs 111121
Painted panels must be incinerated at end-of-life.
3. LCA: Calculation rules
3.1 Declared Unit entirety of the annual production of panels in 2020 and
The functional unit is 1 m2 of acoustic panel, in 35 mm is verified by a third party. Such representativeness is
thickness, corresponding to 13,86 kg of material with a also valid for the production of Portland cement, whose
painted finish, mounted on ceiling, with a reference EPDs, however, were published in 2021 (white) and
service life of 50 years. 2017 (grey). The EPD for the paint used was published
in 2018.
Declared unit
Name Value Unit Temporal, geographical and technological
Declared unit 1 m2 representativeness
Gross density 402 kg/m3 All data strictly related to the cement production is
Grammage 13.86 kg/m2 technologically, temporally, and geographically
Layer thickness 0.035 m representative. The cement production data is less
than 5 years old. However, since the improvement in
grey cement production processes in the meantime
have not been accounted for, the LCA results for the
3.2 System boundary Troldtekt panels based on grey cement can be said to
Cradle to grave be conservative. The data used to model the
foreground inventory of acoustic panels dates from the
3.3 Estimates and assumptions production year of 2020. As for secondary data, some
Assumptions are described occasionally throughout most of the ecoinvent datasets are less than 3 years
the section "LCA: Calculation rules". old.
3.4 Cut-off criteria 3.7 Period under review
The cut-off criterion is applied according to EN The primary data concerned with the manufacture (A1-
15804 Section 6.3.5 and PCR part A Section 5.6. A3) relates to the production year 2020 and the data
All inputs and outputs for which data are available are are based on the volumes produced on an annual
included in the LCA model. Data gaps are filled with basis.
conservative assumptions from average data (when
available) or with generic data and are documented 3.8 Allocation
accordingly. Allocation of production data to the multiple produced
The following product flows have been omitted types of panels (with the same functional unit) is
according to the 1% cut-off rule: performed based on the rules provided in EN 15804.
 Wooden pallet to transport the product Sub-processes associated to painting have specially
been allocated to the painted panels. Data such as
 Capital infrastructure (factory)
waste generation and packaging have been allocated
 Energy utilization of incinerated paint
to the entire production volume of panels in Troldtekt.
 Allocation of burden from wood logging to The only case of co-produced outputs is associated to
residual wood fractions wood logging. However, the environmental load is
evenly distributed over all its co-products, such as
logs, energy wood, and bark.
3.5 Background data
3.9 Comparability
Two types of data source are used as secondary data:
Basically, a comparison or an evaluation of EPD data
 Product-specific EPDs for the manufacture
is only possible if all the data sets to be compared
and supply of Portland cement and water- were created according to EN 15804 and the building
based paint context, respectively the product-specific
 Database ecoinvent v.3.6 cut-off characteristics of performance, are taken into account.
The used background database is ecoinvent v.3.6 cut-
off
3.6 Data quality
Statistical representativeness
The statistical representativeness of the product
system is very good. The input and output data
samples used to build inventories are based on the
4 Environmental Product Declaration Troldtekt A/S – Troldtekt 35mm Natural Grey - painted
4. LCA: Scenarios and additional technical information
Manufacture (A1-A3)
Data
Primary data is third-party verified and based on the Installation into the building (A5)
production year 2020, within the facilities of Troldtekt Name Value Unit
A/S in Jutland (Denmark). Electricity consumption 0,060 kWh
Material loss (plastic film) 0,009 kg
End-of-waste state and use of by-products Material loss (cardborad) 0,039 kg
For all processes supplying a residual material/waste Use phase (B1)
that originates the end-of-life phase of a product to the Prior to distribution and during the use phase (B1), the
product system to be used as input, the polluter-pay carbonation of the cement contained in the panel,
principle “100:0” is used. Some wooden by-products during use, is accounted for. Based on laboratory
generated during manufacture in Troldtekt end up as measurement, the panel will absorb up to 140 grams of
soil improvers externally (reaching end-of-waste state), carbon dioxide per kilogram of cement. Normalized to
and thus their biogenic carbon leaves Troldtekt's the reference flow, this corresponds to an uptake of
system boundary. approximately 0,9 kilograms of carbon dioxide by the
end of the service lifetime, including the uptake in A3.
Wind-certified electricity
All the electricity used to produce the panels in the Maintenance (B2)
Module A3 originates from Danish wind power, for As the panel does not require any maintenance except
which a certificate ensures the origin. It originates from for the occasional dusting, no maintenance module
a 1-3 MW offshore wind turbine, with transformation, (B2) is considered.
transmission and distribution losses and is modelled
correspondingly. Maintenance (B2)
As the panel does not require any maintenance except
Carbon balance for the occasional dusting, no maintenance module
Biogenic: Absorption of biogenic CO 2 by the purchased (B2) is considered.
wood has been considered in A1. Some of it is
released again during production in A3, some ends up
Name Value Unit
sequestered in soil, while the majority of the remaining
biogenic CO , 7,87 kg, is retained in the finished
2 Repair, replacement, refurbishment (B3, B4, B5)
product and emitted during end-of-life incineration in
As the technical service life of the panel is superior to
C4.
the assumed service life of the building (50 years), no
Fossil: Absorption of some fossil CO , originating from
2 repair (B3), replacement (B4) or refurbishment (B5)
the calcination of limestone during cement production,
steps are considered.
happens when the cement is mixed with water in A3. A
majority is absorbed during the use phase B1, and all
the absorbed fossil CO is finally emitted during end- Name Value Unit
2
of-life incineration in C4.
Replacement (B4) / Refurbishment (B5)
Distribution to site (A4) and mounting (A5) Name Value Unit
To consider the main geographical variants of the life
Information about reference service life is detailed in
cycle of Troldtekt Natural Grey panels, three scenarios
2.12.
are developed, where the product is supplied,
mounted, used and discarded in Aarhus (Denmark),
Reference service life
Hamburg (Germany) and Malmö (Sweden). An
Name Value Unit
additional 50 km from the local warehouse to
Reference service life (according to
construction site is assumed. 50 a
ISO 15686-1, -2, -7 and -8)
Life Span (according to BBSR) 50 a
Transport to the building site (A4) Life Span according to the 75 a
manufacturer
Name Value Unit
Litres of fuel 26,8 l/100km
Transport distance to Denmark 160 km Operational energy use (B6) and Operational water
use (B7)
Transport distance to Germany 370 km
Name Value Unit
Transport distance to Sweden 394 km
Water consumption - m3
Transport distance from
Electricity consumption - kWh
warehouse to local construction
50 km Other energy carriers - MJ
sites in
Denmark/Germany/Sweden Equipment output - kW
Capacity utilisation (including
empty runs) 85 % End of life (C1-C4)
Gross density of products Name Value Unit
402 kg/m3 Electricity use (for un-mounting) 0,060 kWh
transported
Transport (to material sorting
Capacity utilisation volume factor 1 - 50 km
facility)
Collected as mixed construction 13,86 kg
5 Environmental Product Declaration Troldtekt A/S – Troldtekt 35mm Natural Grey - painted
waste
Energy recovery 3,98 kg
Energy recovery efficiency 10 %
Energy recovered 8,12 MJ
The panel is un-mounted at the end of its reference
service life and driven to the regional waste
incineration plant. Energy is recovered from the wood
part of the panel at 10% efficiency.
Reuse, recovery and/or recycling potentials (D),
relevant scenario information
Name Value Unit
Electricity 1,93 MJ
Heat 6,19 MJ
The energy substituted from incineration of the panel's
wood component in C4 is considered being a split of
the Danish electricity grid mix (for electricity) and
natural gas (for heat).
Details on possible disposal routes
Aalborg Portland cement factory utilizes dust and
offcuts from the Troldtekt factory as a raw material in
new cement, i.e. in the technical circle. During
incineration in the cement kiln, the wood content in the
cement bonded wood wool panels replaces fossil fuels,
while the cement ends up as a raw material in new
cement, replacing virgin raw materials and heavy fossil
fuels, thereby avoiding a significant amount of CO
2
emissions. This scheme of wood wool waste as a raw
material can be scaled for construction site and
demolition waste. It will be gradually rolled out to all of
Denmark in the period 2021-2023. Once Denmark has
documented economic and environmental benefits to
be gained by including wood wool waste in the
production of new cement rather than going to waste
incineration or landfill, dialogue with municipalities and
local cement producers in the primary markets of
Troldtekt is initiated to facilitate similar schemes
regionally or nationally.
6 Environmental Product Declaration Troldtekt A/S – Troldtekt 35mm Natural Grey - painted
5. LCA: Results
Note: Global Warming Potential (GWP) indicator includes CO of both biogenic and fossil origin.
2
Also, GWP results for Troldtekt Natural Grey (painted) for other delivery scenarios in respectively Germany and
Sweden, are 2,72E-1 kg CO and 2,88E-1 kg CO .
2 2
DESCRIPTION OF THE SYSTEM BOUNDARY (X = INCLUDED IN LCA; MND = MODULE NOT DECLARED;
MNR = MODULE NOT RELEVANT)
BENEFITS AND
CONSTRUCTI LOADS
PRODUCT STAGE ON PROCESS USE STAGE END OF LIFE STAGE BEYOND THE
STAGE SYSTEM
BOUNDARIES
7 Environmental Product Declaration Troldtekt A/S – Troldtekt 35mm Natural Grey - painted
lairetam
waR
ylppus tropsnarT
gnirutcafunaM
eht
morf
tropsnarT
etis
eht
ot
etag
ylbmessA esU
ecnanetniaM
riapeR
tnemecalpeR tnemhsibrufeR
ygrene
lanoitarepO esu
retaw
lanoitarepO esu
noitcurtsnoc-eD
noitilomed tropsnarT
gnissecorp
etsaW
lasopsiD -esueR -yrevoceR -gnilcyceR laitnetop
A1 A2 A3 A4 A5 B1 B2 B3 B4 B5 B6 B7 C1 C2 C3 C4 D
X X X X X X MND MNR MNR MNR MND MND X X MND X X
RESULTS OF THE LCA - ENVIRONMENTAL IMPACT according to EN 15804+A1: 1 m2 Natural Grey, 35
mm, painted finish, delivered and used in Denmark
Parameter Unit A1-A3 A4 A5 B1 C1 C2 C4 D
GWP [kg CO2-Eq.] 2.45E+0 1.36E-1 1.23E-1 -1.00E+0 6.50E-4 1.15E-1 9.20E+0 -1.06E+0
ODP [kg CFC11-Eq.] 3.24E-7 2.48E-8 1.67E-9 0.00E+0 2.81E-10 2.09E-8 7.13E-9 -5.87E-8
AP [kg SO2-Eq.] 2.29E-2 2.75E-4 6.03E-5 0.00E+0 1.59E-6 2.32E-4 5.89E-4 -2.20E-3
EP [kg (PO4)3--Eq.] 7.92E-3 5.65E-5 1.12E-4 0.00E+0 8.86E-7 4.76E-5 2.56E-4 -1.63E-3
POCP [kg ethene-Eq.] 1.14E-3 1.81E-5 2.70E-6 0.00E+0 8.88E-8 1.52E-5 4.61E-5 -1.27E-4
ADPE [kg Sb-Eq.] 5.28E-5 3.71E-6 2.12E-7 0.00E+0 1.82E-8 3.12E-6 7.77E-7 -2.85E-6
ADPF [MJ] 6.06E+1 2.07E+0 3.72E-1 0.00E+0 4.20E-2 1.74E+0 7.12E-1 -1.49E+1
GWP = Global warming potential; ODP = Depletion potential of the stratospheric ozone layer; AP = Acidification potential of land and water; EP =
Caption Eutrophication potential; POCP = Formation potential of tropospheric ozone photochemical oxidants; ADPE = Abiotic depletion potential for non-
fossil resources; ADPF = Abiotic depletion potential for fossil resources
RESULTS OF THE LCA - INDICATORS TO DESCRIBE RESOURCE USE according to EN 15804+A1: 1 m2
Natural Grey, 35 mm, painted finish, delivered and used in Denmark
Parameter Unit A1-A3 A4 A5 B1 C1 C2 C4 D
PERE [MJ] 7.29E+1 2.92E-2 1.60E-1 0.00E+0 3.91E-2 2.46E-2 9.39E+0 -6.95E+0
PERM [MJ] 8.21E+1 0.00E+0 0.00E+0 0.00E+0 0.00E+0 0.00E+0 0.00E+0 0.00E+0
PERT [MJ] 1.55E+2 2.92E-2 1.60E-1 0.00E+0 3.91E-2 2.46E-2 9.39E+0 -6.95E+0
PENRE [MJ] 6.12E+1 2.07E+0 3.72E-1 0.00E+0 4.20E-2 1.74E+0 7.12E-1 -1.49E+1
PENRM [MJ] 1.51E-1 0.00E+0 0.00E+0 0.00E+0 0.00E+0 0.00E+0 0.00E+0 0.00E+0
PENRT [MJ] 6.13E+1 2.07E+0 3.72E-1 0.00E+0 4.20E-2 1.74E+0 7.12E-1 -1.49E+1
SM [kg] 2.92E+0 0.00E+0 0.00E+0 0.00E+0 0.00E+0 0.00E+0 0.00E+0 0.00E+0
RSF [MJ] 6.65E+0 0.00E+0 0.00E+0 0.00E+0 0.00E+0 0.00E+0 0.00E+0 0.00E+0
NRSF [MJ] 7.43E+0 0.00E+0 0.00E+0 0.00E+0 0.00E+0 0.00E+0 0.00E+0 0.00E+0
FW [m³] 5.61E-1 3.54E-4 1.35E-4 0.00E+0 1.19E-5 2.98E-4 3.13E-4 -2.04E-3
PERE = Use of renewable primary energy excluding renewable primary energy resources used as raw materials; PERM = Use of
renewable primary energy resources used as raw materials; PERT = Total use of renewable primary energy resources; PENRE = Use of
non-renewable primary energy excluding non-renewable primary energy resources used as raw materials; PENRM = Use of non-
Caption
renewable primary energy resources used as raw materials; PENRT = Total use of non-renewable primary energy resources; SM = Use
of secondary material; RSF = Use of renewable secondary fuels; NRSF = Use of non-renewable secondary fuels; FW = Use of net fresh
water
RESULTS OF THE LCA – WASTE CATEGORIES AND OUTPUT FLOWS according to EN 15804+A1:
1 m2 Natural Grey, 35 mm, painted finish, delivered and used in Denmark
Parameter Unit A1-A3 A4 A5 B1 C1 C2 C4 D
HWD [kg] 5.68E-2 2.10E-3 1.54E-3 0.00E+0 5.40E-5 1.77E-3 1.64E-3 -6.49E-2
NHWD [kg] 1.93E+0 1.44E-1 1.17E-1 0.00E+0 1.12E-3 1.21E-1 6.90E-2 -2.21E+0
RWD [kg] 1.16E-4 1.42E-5 2.56E-6 0.00E+0 5.78E-7 1.19E-5 5.54E-6 -2.69E-5
CRU [kg] 6.83E-6 0.00E+0 0.00E+0 0.00E+0 0.00E+0 0.00E+0 0.00E+0 0.00E+0
MFR [kg] 1.93E-2 0.00E+0 0.00E+0 0.00E+0 0.00E+0 0.00E+0 0.00E+0 0.00E+0
MER [kg] 1.04E-2 0.00E+0 0.00E+0 0.00E+0 0.00E+0 0.00E+0 0.00E+0 0.00E+0
EEE [MJ] 0.00E+0 0.00E+0 0.00E+0 0.00E+0 0.00E+0 0.00E+0 1.93E+0 0.00E+0
EET [MJ] 0.00E+0 0.00E+0 0.00E+0 0.00E+0 0.00E+0 0.00E+0 6.19E+0 0.00E+0
HWD = Hazardous waste disposed; NHWD = Non-hazardous waste disposed; RWD = Radioactive waste disposed; CRU = Components
Caption for re-use; MFR = Materials for recycling; MER = Materials for energy recovery; EEE = Exported electrical energy; EEE = Exported
thermal energy
6. LCA: Interpretation
The estimated impact results are only relative and use of cement, wood, and paint in the foreground
statements which do not indicate the end points of the processes. Global Warming Potential net emissions
impact categories, exceeding threshold values, safety share is much larger in C4 than in A1-A3 (see why in
margins or risks. chart (2)), while other impact categories in module D in
general are avoided in the waste system owing to the
Two charts are presented: (1) with the standard incineration of end-of-life panels and substitution of
lifecycle impact categories displaying the share of natural gas and Danish electricity mix. C4 also slightly
impacts across all lifecycle stages, and (2) displaying follows emissions of compounds associated to other
the total carbon balance of the Troldtekt product's impact categories. A relatively inefficient transportation
lifecycle system. of end-of-life panels to waste incineration causes
emissions in especially Abiotic depletion of non-fossil
Impacts from the A1-A3 modules are dominant in the resources, Depletion of stratospheric ozone, and
life cycle of the Troldtekt Natural Grey painted panel Photochemical ozone formation.
products. This is primarily caused by the acquisition
The embodied emissions associated to the raw sequestered in A1-A3 and some fossil CO taken up in
2
materials (primarily cement and paint) are the main A1-A3 and B1 is re-emitted in C4. CO emissions
2-eq
cause of impacts, especially in terms of net Global occurring in the remaining modules are negligible.
Warming Potential, with respectively 9,3 kg CO and
2-eq
0,4 kg CO followed by minor impacts from additives. The amount of wood stored in the product refers to a
2-eq
In general, direct emissions from the Troldtekt negative contribution to Global Warming Potential,
production site are relatively small. Abiotic depletion of reducing the share of Global Warming Potential in A1-
fossil resources appears from the burden of producing A3. This is due to the sequestration of biogenic carbon
cement using fossil raw material such as limestone of wood during tree growth. The sequestered carbon
and to a large extent fossil fuels. In terms of carbon does not contribute to global warming as long as it is
balance, biogenic CO in A1-A3 offsets nearly all the stored in the biomass.
2
fossil CO emissions in A1-A3. All biogenic CO
2 2
8 Environmental Product Declaration Troldtekt A/S – Troldtekt 35mm Natural Grey - painted
Summary Global Warming and Eutrophication, by order of
Within the cradle to grave, the following aspects have importance. The treatment of wastewater from the
been identified as major contributors, mainly in the painting cabin also contributes significantly to potential
categories Global Warming Potential and Abiotic impacts in terms of Eutrophication.
depletion of fossil resources:
The clinker (cement) production is the most critical
 Emissions from the clinker production from process of the Troldtekt product system, but
material inaccuracies around the amount used will not
invalidate the present conclusions.
 Emissions from the clinker production from
fuel
Notably, by introducing more up-to-date LCA datasets
 Substituted emissions from end of life for the grey cement applied, or introducing cements
incineration with less carbon footprint into production, as well as
improved paint consumption management, could lead
to significant reductions of especially the Global
Additionally, for painted panels, the manufacture of
Warming Potential indicator.
paint contribute significantly to impacts on potentials
for Photochemical ozone formation, Acidification,
7. Requisite evidence
Technological Institute under DANAK accreditation
7.1 Testing of substances used 392. Report no. MAIC-2019-1418. Reporting of
A detailed assessment of substances used was measured concentrations in toluene equivalents
conducted by a DAkkS-accredited laboratory, based according to EN 16516. This test is basis for the Finish
on a sample (prepared according to EN 15443), M1 Material certificate as well as the Danish Indoor
available in the Test Report 2018P216294, using Climate labeling certificate.
inductively coupled plasma mass spectrometry (EN
16171) and X-ray fluorescence (EN 15309), for the AgBB overview of results (28 days [µg/m³])
following: Name Value Unit
 Heavy metals (cadmium, mercury, etc.) TVOC (C6 - C16) 12 μg/m3
 and other elements Sum SVOC (C16 - C22) 0 - 5 μg/m3
VOC without NIK 0 - 5 μg/m3
Carcinogenic Substances 1 μg/m3
7.2 Leaching
No leaching measurement was conducted according
AgBB overview of results (3 days [µg/m³])
to EN 717-1.
Name Value Unit
TVOC (C6 - C16) - μg/m3
Sum SVOC (C16 - C22) - μg/m3
7.3 VOC emissions
R (dimensionless) - -
Testing for VOC emissions has been conducted in
VOC without NIK - μg/m3
accordance with EN ISO 16000-6. Analysis of the air
Carcinogenic Substances - μg/m3
sampled on Tenax was performed at the Danish
8. References
Standards DIN 52612-2, Testing of thermal insulating materials;
determination of thermal conductivity by means of the
AgBB guarded hot plate apparatus; conversion of the
AgBB, Ausschuss zur gesundheitlichen Bewertung von measured values for building applications. 1 June 1984
Bauprodukten (Committee for Health-related
Evaluation of Building Products) DIN EN ISO 14025
DIN EN ISO 14025:2011, Environmental labels and
BBSR declarations – Type III environmental
BBSR, Bundesinstitut für Bau-, Stadt- und declarations – Principles and procedures, German and
Raumforschung (Federal Institute for Research on English versions EN ISO 14025:2011
Building, Urban Affairs and Spatial Development).
BBSR table: EN 13168
https://www.nachhaltigesbauen.de/fileadmin/pdf/baust EN 13168:2012+A1:2015, Thermal insulation products
off_gebauededaten/BNB_Nutzungsdauern_von_Bautei for buildings. Factory made wood wool (WW) products.
len_2017-02-24.pdf Specification
DIN 4108-4 EN 13964
DIN 4108-4:2017-03, Thermal insulation and energy EN 13964:2014, Suspended ceilings. Requirements
economy in buildings - Part 4: Hygrothermal design and test methods
values
EN 15309
DIN 52612-2 EN 15309:2007, Characterization of waste and soil.
9 Environmental Product Declaration Troldtekt A/S – Troldtekt 35mm Natural Grey - painted
Determination of elemental composition by X-ray ISO 16000-6:2011, Indoor air - Part 6: Determination of
fluorescence volatile organic compounds in indoor and test chamber
air by active sampling on Tenax TA sorbent, thermal
EN 15443 desorption and gas chromatography using MS or MS-
EN 15443:2011, Solid recovered fuels. Methods for the FID
preparation of the laboratory sample
Product Category Rule A
EN 15804 Product Category Rule A, IBU, 2021, Part A,
EN 15804:2012, EN 15804:2012+A1 2013, Calculation Rules for the Life Cycle Assessment and
Sustainability of construction works – Environmental Requirements on the Project Report. v.2.0.1. IBU,
Product Declarations – Core rules for the product 2021.
category of construction products.
Product Category Rule B
EN 16171 Product Category Rule B, IBU, 2019, Part B,
EN 16171:2016, Sludge, treated biowaste and soil. Requirements on the EPD for Wood cement - Mineral-
Determination of elements using inductively coupled bonded wooden composites. v.1.7. IBU, 2019.
plasma mass spectrometry (ICP-MS)
EN 16449 Further References
EN 16449:2014, EN 16449:2014, Wood and wood-
based products - Calculation of the biogenic carbon General Programme Instructions, IBU 2016
content of wood and conversion to carbon dioxide General Programme Instructions for the Preparation of
EPDs at the Institut Bauen und Umwelt e.V. Version 1.,
EN 16516 Berlin: Institut Bauen und Umwelt e.V., 2016.
EN 16516:2017+A1:2020, Construction products:
Assessment of release of dangerous substances. Software/database
Determination of emissions into indoor air OneClick LCA software, Pre-verified EPD tool,
Bionova: https://www.oneclicklca.com/
EN 717-1
EN 717-1:2004, Wood-based Panels – Determination Database: Ecoinvent v.3.6. cut-off (2019)
of Formaldehyde Release – Formaldehyde emission
by the chamber method
ISO 16000-6
10 Environmental Product Declaration Troldtekt A/S – Troldtekt 35mm Natural Grey - painted
Publisher
Institut Bauen und Umwelt e.V. Tel +49 (0)30 3087748- 0
Panoramastr. 1 Fax +49 (0)30 3087748- 29
10178 Berlin Mail info@ibu-epd.com
Germany Web www.ibu-epd.com
Programme holder
Institut Bauen und Umwelt e.V. Tel +49 (0)30 - 3087748- 0
Panoramastr 1 Fax +49 (0)30 – 3087748 - 29
10178 Berlin Mail info@ibu-epd.com
Germany Web www.ibu-epd.com
Author of the Life Cycle
Assessment Tel 98777223
Aalborg Portland Fax 80815733
Rørdalsvej 44 Mail
92200 Aalborg Ø stefan.e.danielsson@cementirhol
Denmark ding.it
Web www.aalborgportland.dk
Owner of the Declaration
Troldtekt A/S Tel +45 8747 8100
Sletvej 2A Fax +45 8747 8111
8310 Tranbjerg J Mail sales@troldtekt.dk
Denmark Web https://www.troldtekt.com
