Publisher: The Norwegian EPD Foundation
Registration number: NEPD-5594-4892-EN
Product Environmental Profile
Product line : TSLF 24-36kV single core
Reference product : TSLF-M 24kV 1x240A
EDS 1147
Product Category Rules: PEP-PCR-ed3-EN-2015 04 02
PEP ecopassport N°: NXNS-00094-V01.01-EN
Product Specific Rules: PSR-0001-ed3-EN-2015 10 16
Verifier accreditation n°: VH18 Program information & documents: www.pep-ecopassport.org
Date of publication: 05-2021 Validity period: 5 years
Independent verification of the declaration and data, in accordance with ISO 14025 : 2010
Internal o External 
The PCR critical review was conducted by a panel of experts chaired by Philippe Osset (Solinnen).
PEP are compliant with XP C08-100-1 :2016
The elements of the present PEP cannot be compared with elements from another program.
Compliant with ISO 14025: 2010 "Environmental labels and declarations - Type III environmental declarations".
Compliant with the mutual recognition agreement of 2023/07/05 between PEP Ecopassport and Epd-Norge.
Realized by: Jan Erik Nilsen
Postboks 100, 1403 Langhus - Norway
8 jan_erik.nilsen@nexans.com ) +47 64861988 : www.nexans.com/sustainable
PEP ecopassport N° NXNS-00094-V01.01-EN
FOR-58001 issue 21 Crédits : © Nexans, Fotolia 1
I. PRODUCTS AND COMMITMENT
Nexans Environmental commitments
Nexans integrates Sustainable Development in its strategy to meet stakeholders needs. Nexans has
been supporting the United Nations Global Compact since December 2008 and has implemented
internal action plans to integrate Sustainable Development at all levels: responsible governance,
healthy and safe working environment for employees, setting up carbon footprint of Nexans sites,and
designing high performance products.
Reference Product description
TSLF-M 24kV 1x240A
TSLF is a longitudinally and radially waterblocked, XLPE -insulated, copper wire screened, PE sheathed single core cable with circular
aluminium conductor. The outer conductive layer on the insulation is crosslinked vulcanized elastomer. The cable may be used for fixed
installation outdoors in air, ground and water and is designed according to HD 620 10K.
Products covered:
The aforementioned products belong to the category Wires, Cables and Accessories of the Product Category Rules (PCR) from the
PEP ecopassport® program.
ThePEPconcernalltheproductsintherange TSLF24-36kVsinglecoreand thereferenceproductofthePEPisthe productTSLF-M
24kV 1x240A.
Functional unit:
To transmit energy expressed for 1 A over a distance of 1 km during 40 years and a 100% use rate, in accordance with the relevant
standards, detailed in the data sheet available on our website www.nexans.com.
Lifetime and use rate correspond to the Infrastructure - Power networks application as defined in the table given in Appendix1 of the
specific rules for wires, cables and accessories.
This PEP has been drawn up considering the following parameters:
-1 km for manufacturing, distribution and end-of-life stages
-1 km and 1 A for the use stage;
ThepotentialimpactoftheusestageshallbecalculatedbythePEPuserconsideringtherealamperagethroughtheproductduringthe
use by multiplying the impact by the square of the intensity. This PEP is valid in the intensity range taking into account the maximum
allowable intensity.
Materials and substances
The total mass of the reference product and packaging is 2001,33 kg/km. Constituent materials are distributed as follows:
• 35,5% Plastics including 1,2% of recycled plastic for the product (7% of recycled PE in the sheath).
• 41,1% Metals
• 23,4% Others
PEP ecopassport N° NXNS-00094-V01.01-EN
FOR-58001 issue 21 Crédits : © Nexans, Fotolia 2
II. LIFE CYCLE ASSESSMENT
Manufacturing
 All the products in the range TSLF 24-36kV single core are manufactured in France and in Norway.
 The electricity mix model for the manufacturing stage is France, >1 kV and Norway, >1 kV.
 AllNexanssitesinNorwayandinFrancehaveimplementedacertifiedEnvironmentalManagementSystemaccordingtoISO14001
standard.
Packaging designed to reduce environmental impacts:
Packaging was designed according to the applicable standard (Directive 94/62/EC).
 The packaging considered to transport the reference product is a Wooden drum. It is considered to be used 1 time.
 The considered packaging is a PEFC™ (Programme for the Endorsement of Forest Certification) certified wooden drum, ensuring
responsible sourcing and sustainable forests management.
In Norway,Nexans has developed a collecting system for NXdrums typecalled Tromløp,a NexansTrommelservice. Returning drums
canbemadebyphone(64861900),bye-mail(norge.trommelretur@nexans.com),byinternet(www.nexans.no/eservice)orbymobile
application (EASYREEL™).
Distribution
The transportation scenario for the impact assessment of the distribution stage is local (Norway), considering:
 1000 km covered by truck.
Installation
Installation processes for the reference product are considered out of the scope of the study, according to the Product Specific Rules
document for "Wires, Cables and Accessories" from PEP ecopassport® program. Only packaging disposal is considered at this stage.
Use
 The use scenario considers the operation of the reference product in Infrastructure / Power networks, with:
• Reference Lifetime (RLT) = 40 years • Use rate = 100 %
• Current intensity (A): 1 • Cable resistance* (ohm/km):0,125 • Number of active conductor(s): 1
(*According to standard IEC 60228)
 Considering the aforementioned hypotheses, the energy consumption over the RLT at use stage is 43,8 kWh/km.
This value is calculated for I=1 A. For the effective consumption of the cable installed, multiply the value given by the square intensity.
 The electricity mix considered at use stage is Norway, <1 kV.
 No maintenance is necessary to ensure the operation of the cable during the considered reference lifetime.
The reference lifetime mentioned in this PEP corresponds to an average data used for impact calculation, taking into account the
average time a cable might be installed in a system before being disposed. It CANNOT BE considered as an equivalent to the
guaranteed product technical lifetime.
End-of-life
 The transportation scenario chosen for the impact analysis associated with end-of-life stage is 1000 km covered by truck.
 The assumed electricity mix model for end-of-life stage is Norway, >1 kV.
The cables are recycled through a grinding process for the separation of polymers and metal parts. It was considered that 100% of
metals are recycled and 100% of other materials are landfilled.
Nexans has the know-how of cables recycling at their end-of-life through the structure named Nexans Recycling Services
(recycling.services@nexans.com), to offer a complete solution for the recycling of polymers and metals.
PEP ecopassport N° NXNS-00094-V01.01-EN
FOR-58001 issue 21 Crédits : © Nexans, Fotolia 3
Total use of primary
MJ 1,70E+05 1,41E+03 3,08E+02
energy
Net fresh water use m3 4,63E+03 8,92E-03 7,01E-03 4,12E+02 2,37E+03 7,41E+03
*Installation stage includes only packaging disposal. Impacts related to installation processes might be completed by the PEP user.
yrotnevnI
swolf
III. ENVIRONMENTAL IMPACTS
The reference product TSLF-M 24kV 1x240A belongs to the category Wires, Cables and Accessories of the Product Category Rules
(PEP-PCR-ed3-EN-2015 04 02) from the PEP ecopassport® program. According to the PCR, the life cycle impact assessment of the
reference product takes into account manufacturing, distribution, installation, use and end-of-life stages.
All the necessary hypotheses to evaluate the environmental impacts of the reference product lifecycle are presented in the previous
sections (electricitymixmodels,use scenario, etc).The software used to perform the evaluation is EIME 5.9.1,with theNexans-2021-
02 database.
Representativeness: the study is representative of cable production in Norway with a local scenario for distribution. The electricity
model for use is Norway, <1 kV and the model for end-of-life is Norway, >1 kV.
Impact results for 1000 m of TSLF-M 24kV 1x240A
Indicators/ Flows Unit Manufacturing Distribution Installation* Use End-of-life TOTAL
(for 1 A) (for 1 A)
2,24E+01 1,03E+00 1,39E+02 9,59E+03
kg CFC-
Ozone Depletion 2,04E-03 2,02E-07 1,53E-07 2,02E-09 2,30E-06 2,04E-03
11 eq.
Acidification of soils and kg SO
2 6,02E+01 4,48E-01 1,10E-01 1,18E-03 5,47E-01 6,13E+01
water eq.
kg PO 3- Water Eutrophication 4 3,79E+00 1,03E-01 1,19E-01 1,44E-04 4,49E-01 4,46E+00
eq.
Photochemical Ozone kg C H
2 4 3,28E+00 3,18E-02 7,76E-03 9,65E-05 4,12E-02 3,36E+00
formation eq.
Depletion of abiotic
kg Sb eq. 2,27E-01 3,99E-06 9,75E-07 8,84E-06 5,83E-05 2,27E-01
resources (elements)
2,14E+02 2,83E+03 1,75E+05
srotacidni
tcapmi
latnemnorivnE
kg CO
Global Warming 2 9,33E+03 9,96E+01
eq.
PEP ecopassport N° NXNS-00094-V01.01-EN
FOR-58001 issue 21 Crédits : © Nexans, Fotolia 4
Materials for energy
kg 0,00E+00 0,00E+00 0,00E+00 0,00E+00 0,00E+00 0,00E+00
recovery
0,00E+00 0,00E+00 8,17E+02 8,47E+02
tuptuO
-
swolf
yrotnevnI
swolf
Use of secondary
kg 8,65E+01 0,00E+00 0,00E+00 0,00E+00 0,00E+00 8,65E+01
materials
1,88E+01
Components for reuse kg 0,00E+00 0,00E+00 0,00E+00 0,00E+00 0,00E+00 0,00E+00
Exported energy MJ 0,00E+00 0,00E+00 0,00E+00 0,00E+00 0,00E+00 0,00E+00
Materials for recycling kg 2,94E+01 0,00E+00
-
swolf
yrotnevnI
slairetam
.dnoceS
Use of renewable
MJ 0,00E+00 0,00E+00
secondary fuels
Use of non-renewable
MJ 0,00E+00 0,00E+00 0,00E+00 0,00E+00 0,00E+00
secondary fuels
3,44E-02 6,00E-01 2,16E+04
Non-hazardous waste
kg 1,86E+04 3,54E+00 3,71E+02 2,75E+00 9,26E+02 1,99E+04
disposed
-
swolf
yrotnevnI
etsaW
5,00E+00 1,52E+03 1,02E+05
Water pollution m3 5,93E+05 1,64E+04 3,47E+03 1,62E+01 1,75E+04 6,30E+05
1,28E+04 1,83E+06
0,00E+00 0,00E+00 0,00E+00 0,00E+00 5,42E+03
Total use of renewable
primary energy MJ 1,37E+04 1,88E+00 3,53E+00 2,06E+02 1,21E+03 1,51E+04
resources
Use of non-renewable
primary energy
MJ 1,26E+05 1,41E+03 3,05E+02 8,90E+00 1,62E+03 1,29E+05
(excluding resources
used as raw materials)
Use of non-renewable
primary energy
MJ 3,04E+04 0,00E+00 0,00E+00 0,00E+00 0,00E+00 3,04E+04
resources used as raw
materials
Total use of non-
renewable primary MJ 1,56E+05 1,41E+03 3,05E+02 8,90E+00 1,62E+03 1,60E+05
energy resources
0,00E+00 0,00E+00 0,00E+00 0,00E+00
0,00E+00
Hazardous waste
kg 2,16E+04 0,00E+00 8,19E-02
disposed
Radioactive waste
kg 1,88E+01 2,52E-03 1,91E-03 1,60E-03 3,73E-02
disposed
secruoser
yramirp
fo
esU
-
swolf
yrotnevnI
III. ENVIRONMENTAL IMPACTS
Indicators/ Flows Unit Manufacturing Distribution Installation Use End-of-life TOTAL
(for 1 A) (for 1 A)
Air pollution m3 1,81E+06 4,08E+03 2,84E+03 2,48E+01
Use of renewable
primary energy
MJ 8,26E+03 1,88E+00 3,53E+00 2,06E+02 1,21E+03 9,68E+03
(excluding resources
used as raw materials)
Use of renewable
primary energy
MJ 5,42E+03
resources used as raw
materials
latnemnorivnE
srotacidni
tcapmi
Depletion of abiotic
MJ 9,87E+04 1,40E+03 3,00E+02
resources (fossil fuels)
PEP ecopassport N° NXNS-00094-V01.01-EN
FOR-58001 issue 21 Crédits : © Nexans, Fotolia 5
IV. EXTRAPOLATION RULES FOR THE PRODUCT LINE TSLF 24-36kV single core
General information
Theextrapolationruleshavebeencalculatedbasedontheenvironmentimpactassessmentresultsof6productsintherangeTSLF24-
36kV single core. The reference product is TSLF-M 24kV 1x240A.
The extrapolation rules below apply to 1000m of product. In the following sections, the product weight is expressed in kg for 1000m of
cable, where applicable.
Manufacturing
The extrapolation principle applicable to manufacturing stage impacts is a Linear variation versus weight.
Each environmental indicator value shall be calculated using the following formula:
Indicator = (a1/a2) x Cable weight + (b1/b2)
N.B.: extrapolation coefficients are different depending on whether the product weight is higher or lower than 1415 kg/km.
Table to be used for manufacturing stage
Weight>1415 kg/km Weight<1415 kg/km
a1 b1 a2 b2
GWP 4,40E+00 2,96E+03 6,30E+00 -1,27E+03
ODP 1,08E-06 4,79E-04 1,37E-06 -2,69E-04
A 2,88E-02 1,92E+01 4,25E-02 -1,16E+01
EP 1,82E-03 1,13E+00 2,57E-03 -5,36E-01
POCP 1,55E-03 1,04E+00 2,26E-03 -5,39E-01
ADPe 9,53E-05 4,95E-02 1,29E-04 1,69E-02
TPE 8,52E+01 4,45E+04 1,09E+02 -1,15E+04
FW 2,97E+00 3,09E+02 1,67E+00 2,03E+03
ADPf 4,58E+01 3,06E+04 6,16E+01 -4,34E+03
WP 2,88E+02 1,75E+05 4,02E+02 -8,93E+04
AP 8,14E+02 4,94E+05 1,16E+03 -1,16E+05
PERE 3,35E+00 3,90E+03 5,45E+00 -9,38E+02
PERM 4,56E+00 -2,72E+03 2,80E+00 9,15E+02
PERT 7,90E+00 1,19E+03 8,26E+00 -2,29E+01
PENRE 6,54E+01 3,23E+04 8,67E+01 -2,00E+04
PENRM 1,19E+01 1,10E+04 1,37E+01 8,48E+03
PENRT 7,73E+01 4,33E+04 1,00E+02 -1,15E+04
RSF 0,00E+00 0,00E+00 0,00E+00 0,00E+00
NRSF 0,00E+00 0,00E+00 0,00E+00 0,00E+00
SM 3,36E-02 2,93E+01 4,09E-02 1,94E+01
HWD 9,13E+00 4,80E+03 1,24E+01 1,36E+03
NHWD 9,11E+00 5,86E+03 1,35E+01 -4,42E+03
RWD 1,08E-02 3,55E+00 1,28E-02 -2,66E+00
CRU 0,00E+00 0,00E+00 0,00E+00 0,00E+00
EE 0,00E+00 0,00E+00 0,00E+00 0,00E+00
MER 0,00E+00 0,00E+00 0,00E+00 0,00E+00
MFR 5,86E-02 -6,99E+01 7,67E-03 9,44E+00
Example: If the product weight is 1650 kg/km, each indicator value shall be calculated with: 1650 x a1 + b1.
The reckoned mean and maximum deviations concerning manufacturing impact extrapolation rules are respectively 4,86% and 17,67%.
PEP ecopassport N° NXNS-00094-V01.01-EN
FOR-58001 issue 21 Crédits : © Nexans, Fotolia 6
IV. EXTRAPOLATION RULES FOR THE PRODUCT LINE TSLF 24-36kV single core
Distribution
The extrapolation principle applicable to distribution stage impacts is a Linear variation versus weight.
Each environmental indicator value shall be calculated using the following formula:
Indicator = a x Cable weight + b
Example:
If the product weight is 1650 kg/km, each indicator value shall be calculated with: 1650 x a + b.
The reckoned mean and maximum deviations concerning distribution impact extrapolation rules are respectively 1,96% and 3,68%.
PEP ecopassport N° NXNS-00094-V01.01-EN
FOR-58001 issue 21 Crédits : © Nexans, Fotolia 7
IV. EXTRAPOLATION RULES FOR THE PRODUCT LINE TSLF 24-36kV single core
Installation
The extrapolation principle applicable to installation stage impacts is a Maximum impact value.
The maximum impact values indicated in the table below are applicable to the whole range for installation stage impacts.
Table to be used for installation phase
Impact
value
GWP 5,03E+01
ODP 3,43E-07
A 2,47E-01
EP 2,66E-01
POCP 1,74E-02
ADPe 2,18E-06
TPE 6,91E+02
FW 1,57E-02
ADPf 6,71E+02
WP 7,78E+03
AP 6,35E+03
PERE 7,90E+00
PERM 0,00E+00
PERT 7,90E+00
PENRE 6,83E+02
PENRM 0,00E+00
PENRT 6,83E+02
RSF 0,00E+00
NRSF 0,00E+00
SM 0,00E+00
HWD 1,84E-01
NHWD 8,32E+02
RWD 4,28E-03
CRU 0,00E+00
EE 0,00E+00
MER 0,00E+00
MFR 0,00E+00
N.B.: Installation stage represents only the disposal of the packaging of the products. Installation processes are excluded from the
system boundaries.
PEP ecopassport N° NXNS-00094-V01.01-EN
FOR-58001 issue 21 Crédits : © Nexans, Fotolia 8
IV. EXTRAPOLATION RULES FOR THE PRODUCT LINE TSLF 24-36kV single core
Use
The extrapolation principle applicable to use stage impacts is a Variation versus resistivity ratio.
The reference product for resistivity ratio is TSLF-M 24kV 1x240A with 1 active conductor(s) and a resistivity of 0,125 ohm/km/active
conductor.
Each environmental indicator value shall be calculated using the following formula:
Indicator = (Product Resistivity / Reference product Resistivity) x Indicator value for Reference Product x (Nb of active
conductors / Nb of active conductors in the reference product)
Example:
If the product resistivity is 1,2 ohm/km, the resistivity ratio shall be calculated as: 1,2/0,125.
Then,tocalculatetheenvironmentalimpactofaproduct,eachimpactindicatorvalueoftheusestageofthereferenceproductshallbe
multiplied by the resistivity ratio and by the ratio of active conductors.
The reckoned mean and maximum deviations concerning use impact extrapolation rules are respectively 0,00% and 0,01%.
PEP ecopassport N° NXNS-00094-V01.01-EN
FOR-58001 issue 21 Crédits : © Nexans, Fotolia 9
IV. EXTRAPOLATION RULES FOR THE PRODUCT LINE TSLF 24-36kV single core
End-of-life
The extrapolation principle applicable to end-of-life stage impacts is a Linear variation versus weight.
Each environmental indicator value shall be calculated using the following formula:
Indicator = a x Cable weight + b
Table to be used for end-of-life stage
a b
GWP 7,84E-02 1,12E+01
ODP 1,15E-09 4,67E-07
A 3,13E-04 3,86E-02
EP 2,30E-04 8,17E-02
POCP 2,34E-05 3,23E-03
ADPe 3,51E-08 9,06E-07
TPE 1,67E+00 9,80E+01
FW 1,44E+00 3,67E-02
ADPf 8,86E-01 7,65E+01
WP 1,02E+01 8,73E+02
AP 6,67E+00 2,07E+03
PERE 7,34E-01 5,20E+00
PERM 0,00E+00 0,00E+00
PERT 7,34E-01 5,20E+00
PENRE 9,39E-01 9,28E+01
PENRM 0,00E+00 0,00E+00
PENRT 9,39E-01 9,28E+01
RSF 0,00E+00 0,00E+00
NRSF 0,00E+00 0,00E+00
SM 0,00E+00 0,00E+00
HWD 3,17E-04 8,95E-02
NHWD 4,54E-01 2,07E+02
RWD 1,96E-05 5,83E-03
CRU 0,00E+00 0,00E+00
EE 0,00E+00 0,00E+00
MER 0,00E+00 0,00E+00
MFR 5,99E-01 -1,88E+02
Example:
If the product weight is 1650 kg/km, each indicator value shall be calculated with: 1650 x a + b.
The reckoned mean and maximum deviations concerning end-of-life impact extrapolation rules are respectively 1,52% and 11,02%.
PEP ecopassport N° NXNS-00094-V01.01-EN
FOR-58001 issue 21 Crédits : © Nexans, Fotolia 10
IV. EXTRAPOLATION RULES FOR THE PRODUCT LINE TSLF 24-36kV single core
Terms and abbreviations
The various abbreviations used in the PEP document are explained in the table below:
Abbreviations Environmental indicator/flow complete name
GWP Global Warming
ODP Ozone Depletion
A Acidification of soil and water
EP Eutrophication
POCP Photochemical Ozone Creation
ADPe Depletion of abiotic resources - elements
TPE Total use of Primary Energy
FW Net use of Freshwater
ADPf Depletion of abiotic resources - fossil fuels
WP Water Pollution
AP Air Pollution
PERE Use of renewable primary energy, excluding renewable primary energy resources used as raw materials
PERM Use of renewable primary energy resources as raw materials
PERT Total use of renewable primary energy resources (PERE+PERM)
PENRE Use of non-renewable primary energy, excluding non-renewable primary energy resources used as raw materials
PENRM Use of non-renewable primary energy resources as raw materials
PENRT Total use of non-renewable primary energy resources (PENRE+PENRM)
RSF Use of renewable secondary fuels
NRSF Use of non-renewable secondary fuels
SM Use of secondary materials
HWD Hazardous waste disposed
NHWD Non-hazardous waste disposed
RWD Radioactive waste disposed
CRU Components for reuse
EE Exported energy
MER Materials for energy recovery
MFR Materials for recycling
PEP ecopassport N° NXNS-00094-V01.01-EN
FOR-58001 issue 21 Crédits : © Nexans, Fotolia 11
Emission factor for electricity mix
The electricity mix model for the manufacturing stage is France, >1 kV and Norway, >1 kV. The emission factors are the following :
-France : 0,0292 kg CO eq. / kwh (ELCD - Provision of medium voltage (1kV - 60kV) electricity for final consumer).
2
-Norway : 0,00612 kg CO eq. / kwh (ELCD - Provision of medium voltage (1kV - 60kV) electricity for final consumer).
2
Content of hazardous substances
The product contains no substances given by the REACH Candidate list or the Norwegian priority list.
Cut-Off criteria
All major raw materials and all the essential energy is included. Less than 1% of the production processes for raw materials and energy
flows are not included. These cut-off criteria do not apply for hazardous materials and substances.
Impact results for 1 m of TSLF-M 24kV 1x240A
Indicators/ Flows Unit
9,65E-08 4,12E-05
srotacidni
tcapmi
latnemnorivnE
Global Warming kg CO eq.
2
kg CFC-11
Ozone Depletion
eq.
Acidification of soils and
kg SO eq.
water 2
3,28E-03
2,27E-04
1,70E+02
4,63E+00
yrotnevnI
swolf
ANNEX - MUTUAL RECOGNITION WITH EDP NORGE
Environmental impacts
Use Module
Manufacturing Distribution Installation* End-of-life TOTAL
(for 1 A) D**
9,33E+00 9,96E-02 2,24E-02 1,03E-03 1,39E-01 9,59E+00 -6,7E+00
2,04E-06 2,02E-10 1,53E-10 2,02E-12 2,30E-09 6,13E-02 -4,5E-02
6,02E-02 4,48E-04 1,10E-04 1,18E-06 5,47E-04 6,13E-02 -4,2E-02
kg PO3- Water Eutrophication 4 3,79E-03 1,03E-04 1,19E-04 1,44E-07 4,49E-04 4,46E-03 -2,6E-03
eq.
Photochemical Ozone kg CH
2 4 3,18E-05 7,76E-06 3,36E-03 -2,2E-03
formation eq.
Depletion of abiotic
kg Sb eq. 3,99E-09 9,75E-10 8,84E-09 5,83E-08 2,27E-04 -2,3E-04
resources (elements)
Total use of primary
MJ 1,41E+00 3,08E-01 2,14E-01 2,83E+00 1,75E+02 -9,9E+01
energy
Net fresh water use m3 8,92E-06 7,01E-06 4,12E-01 2,37E+00 7,41E+00 -1,0E-01
PEP ecopassport N° NXNS-00094-V01.01-EN
FOR-58001 issue 21 Crédits : © Nexans, Fotolia 12
Use Module
Indicators/ Flows Unit Manufacturing Distribution Installation* End-of-life TOTAL
(for 1 A) D**
Radioactive waste
kg 1,88E-02 -1,3E-02
disposed
0,00E+00 0,00E+00 0,00E+00 0,00E+00 0,00E+00 0,00E+00 0,0E+00
0,00E+00 0,0E+00
0,00E+00 0,0E+00
8,47E-01 0,0E+00
*Installation stage includes only packaging disposal. Impacts related to installation processes might be completed by the PEP user.
tuptuO
-
swolf
yrotnevnI
swolf
Use of renewable
MJ
secondary fuels
Use of non-renewable
MJ 0,00E+00 0,00E+00 0,00E+00 0,00E+00 0,00E+00
secondary fuels
8,65E-02 0,00E+00 0,00E+00 0,00E+00
Components for reuse kg
Exported energy MJ 0,00E+00 0,00E+00 0,00E+00 0,00E+00 0,00E+00
Materials for energy
kg 0,00E+00 0,00E+00 0,00E+00 0,00E+00 0,00E+00
recovery
Materials for recycling kg 2,94E-02 0,00E+00 0,00E+00 0,00E+00 8,17E-01
-
swolf
yrotnevnI
etsaW
Use of secondary
kg
materials
Hazardous waste
kg
disposed
-
swolf
yrotnevnI
slairetam
.dnoceS
8,26E+00 1,88E-03 3,53E-03 2,06E-01 1,21E+00
2,16E+01
Non-hazardous waste
kg 1,86E+01
disposed
1,88E-02 2,52E-06 1,91E-06 1,60E-06 3,73E-05
secruoser
yramirp
fo
esU
-
swolf
yrotnevnI
Use of renewable
primary energy
MJ
(excluding resources
used as raw materials)
Use of renewable
primary energy
MJ 5,42E+00 0,00E+00 0,00E+00 0,00E+00 0,00E+00
resources used as raw
materials
Total use of renewable
primary energy MJ 1,37E+01 1,88E-03 3,53E-03 2,06E-01
resources
Use of non-renewable
primary energy
MJ 1,26E+02 1,41E+00
(excluding resources
used as raw materials)
Use of non-renewable
primary energy
MJ
resources used as raw
materials
Total use of non-
renewable primary MJ 1,56E+02 1,41E+00 3,05E-01
energy resources
latnemnorivnE
srotacidni
tcapmi
Depletion of abiotic
MJ 9,87E+01 1,40E+00 3,00E-01 5,00E-03 1,52E+00 1,02E+02 -5,5E+01
resources (fossil fuels)
Water pollution m3 5,93E+02 1,64E+01 3,47E+00 1,62E-02 1,75E+01 6,30E+02 -4,5E+02
Air pollution m3 1,81E+03 4,08E+00 2,84E+00 2,48E-02 1,28E+01 1,83E+03 -1,5E+03
9,68E+00 -6,8E+00
5,42E+00 0,0E+00
1,21E+00 1,51E+01 -6,8E+00
3,05E-01 8,90E-03 1,62E+00 1,29E+02 -9,2E+01
3,04E+01 0,00E+00 0,00E+00 0,00E+00 0,00E+00 3,04E+01 0,0E+00
8,90E-03 1,62E+00 1,60E+02 -9,2E+01
0,00E+00 0,00E+00 0,00E+00 0,00E+00 0,00E+00 0,00E+00 0,0E+00
0,00E+00 0,0E+00
0,00E+00 8,65E-02 -3,0E-02
0,00E+00 8,19E-05 3,44E-05 6,00E-04 2,16E+01 -2,2E+01
3,54E-03 3,71E-01 2,75E-03 9,26E-01 1,99E+01 -1,7E+01
** The recyclability of metals allows the producers a credit for the net scrap that is produced at the end of a product’s life. The benefits from recycling of
net scrap are described in formula from EN 15804:2012+A2:2019. However, the substitution of heat and electricity generated by the incineration with
energy recovery of plastic is uncertain and is therfore not included in module D for the curent case.
PEP ecopassport N° NXNS-00094-V01.01-EN
FOR-58001 issue 21 Crédits : © Nexans, Fotolia 13
Products covered by the family range
Number of active Resistivity
Product Reference Weight (kg/km)
conductors (Ohm/km)
TSLF 24kV 1x50A 10163157 1 684 0,641
TSLF 24kV 1x95A 10163158 1 953 0,32
TSLF 24kV 1x150A 10163159 1 1190 0,206
TSLF 24kV 1x240A 10163160 1 1640 0,125
TSLF 24kV 1x400A 10057165 1 2230 0,0778
TSLF 24kV 1x630A 10060895 1 3170 0,0469
TSLF-M 24kV 1x50A (with red marking stripe) 10548312 1 684 0,641
TSLF-M 24kV 1x95A (with red marking stripe) 10548314 1 953 0,32
TSLF-M 24kV 1x150A (with red marking stripe) 10548315 1 1190 0,206
TSLF-M 24kV 1x240A (with red marking stripe) 10548316 1 1640 0,125
TSLF-M 24kV 1x400A (with red marking stripe) 10548318 1 2230 0,0778
TSLF-M 24kV 1x630A (with red marking stripe) 10548319 1 3170 0,0469
The technical datasheets of all products covered by this PEP are available on the internet link :
https://www.nexans.no/eservice/Norway-en/navigate_372886/TSLF_24_36kV_single_core.html
PEP ecopassport N° NXNS-00094-V01.01-EN
FOR-58001 issue 21 Crédits : © Nexans, Fotolia 14
