ENVIRONMENTAL PRODUCT DECLARATION
as per ISO 14025 and EN 15804+A1
Owner of the Declaration Interface Europe Manufacturing BV
Programme holder Institut Bauen und Umwelt e.V. (IBU)
Publisher Institut Bauen und Umwelt e.V. (IBU)
Declaration number EPD-INT-20200180-CCC1-EN
Issue date 05.11.2020
Valid to 04.11.2025
Modular carpet tiles with CQuest Bio backing
pile material solution dyed polyamide 6.6 with 75% recycled
content and a maximum total pile weight of 1000 g/m2
Interface®
www.ibu-epd.com | https://epd-online.com
Umwelt Produktdeklaration Name des Herstellers – Name des Produkts
General Information
Interface® Modular carpet tiles with CQuest
Bio backing
pile material solution-dyed PA 6.6 with
75% recycled content and a maximum
total pile weight of 1000 g/m2
Programme holder Owner of the declaration
IBU – Institut Bauen und Umwelt e.V. Interface Europe Manufacturing BV
Panoramastr. 1 Industrielaan 15
10178 Berlin 3925 ZG Scherpenzeel
Germany The Netherlands
Declaration number Declared product / declared unit
EPD-INT-20200180-CCC1-EN 1 m² tufted modular carpet tiles with CQuest Bio
backing (CQB) and a pile material of PA 6.6 with 75%
recycled content
This declaration is based on the product Scope:
category rules: The manufacturer declaration applies to modular
Floor coverings, 02/2018 carpet tiles with CQuest Bio backing, a pile material of
(PCR checked and approved by the SVR) PA 6.6 with 75% recycled content and a maximum total
pile weight of 1000 g/m2. The products are tufted in
Craigavon (Ireland). They are back coated in
Issue date
Scherpenzeel.
05.11.2020
LCA results for products with a maximum total pile
weight of 600 g/m2 can be taken from the
Valid to
corresponding tables of the annexe. Specific data for
04.11.2025 every product within the declared group of products in
relation to its total pile weight can be calculated by
using equation 1 given in the annexe (see annexe
chapter: 'General Information on the annexe').
The declaration is only valid in conjunction with a valid
GUT-PRODIS license of the product.
The owner of the declaration shall be liable for the
underlying information and evidence; the IBU shall not
be liable with respect to manufacturer information, life
cycle assessment data and evidences.
The EPD was created according to the specifications
of EN 15804+A1. In the following, the standard will be
simplified as EN 15804.
Verification
The standard EN 15804 serves as the core PCR
Independent verification of the declaration and data
according to ISO 14025:2010
Dipl. Ing. Hans Peters internally x externally
(chairman of Institut Bauen und Umwelt e.V.)
Dr. Alexander Röder Dr. Frank Werner
(Managing Director Institut Bauen und Umwelt e.V.)) (Independent verifier)
Product
Information about the enterprise way that is restorative to the planet and creates a
Interface, Inc. is a global flooring company specializing climate fit for life.
in carbon neutral carpet tile and resilient flooring,
including luxury vinyl tile (LVT) and nora® rubber Product description/Product definition
flooring. We help our customers create high- Tufted modular carpet tiles having a surface pile of
performance interior spaces that support well-being, solution-dyed polyamide 6.6 with 75% recycled content
productivity, and creativity, as well as the sustainability and a CQuest Bio backing system.
of the planet. Our mission, Climate Take Back™,
invites you to join us as we commit to operating in a
2 Environmental Product Declaration Interface – Tufted modular carpet tiles with CQuest Bio backing and a pile material of
PA 6.6 with 75% recycled content
CQuest Bio backing system:
Backing compound based on wood resin, containing
recycled filler, glass-fleece reinforcement and Performance data of the product in accordance with
polypropylene covering fleece. the declaration of performance with respect to its
The minimum recycled content out of total weight is essential characteristics according to EN 14041.
75%. Additional product properties in accordance with EN
The declaration applies to a group of products with a 1307 can be found on the Product Information System
maximum total pile weight of 1000 g/m2. PRODIS using the PRODIS registration number of the
LCA results for products with a maximum total pile product (www.pro-dis.info) or on the manufacturer's
weight of 600 g/m2 can be taken from the technical information section (www.interface.com).
corresponding tables of the annexe. Results for
specific products with any other total pile weight can be Base materials/Ancillary materials
calculated by using equation 1 given in the annexe
(see annexe chapter: 'General Information on the Name Value Unit
annexe'). Polyamide 6.6 22.6 %
For the placing on the market of the product in the Polyester 2.7 %
European Union/European Free Trade Association Polypropylene 1.1 %
(EU/EFTA) (with the exception of Switzerland) Limestone 52.6 %
Regulation (EU) No. 305/2011 Construction Product Aluminum hydroxide 5.5 %
Regulation (CPR) applies. The product needs a Ethylene vinyl acetate (EVA) 6.2 %
Declaration of Performance (DoP) taking into Wood resin 6.5 %
consideration EN 14041 and the CE-marking. The DoP
Glass fibre 0.8 %
of the product can be found on the manufacturer's
Additives 2.0 %
technical information section. For the application and
use of the product the respective national provisions
The products are registered in the GUT-PRODIS
apply.
Information System. The PRODIS system ensures the
compliance with limitations of various chemicals and
Application
Volatile Organic Compound (VOC)-emissions and a
According to the use class as defined in EN 1307 the
ban on the use of all substances that are listed as
products can be used in all professional areas which
'Substances of Very High Concern' (SVHC) under
require class 33 or less.
REACH.
This product contains substances listed in the ECHA
candidate list (16.01.2020) exceeding 0.1 percentage
by mass: no
Technical Data
The performance data listed in the DoP apply. Reference service life
A calculation of the reference service life according to
Name Value Unit ISO 15686 is not possible.
Modular carpet tiles, The service life of textile floor coverings strongly
Product Form -
50 cm x 50 cm depends on the correct installation taking into account
Type of manufacture tufted carpet - the declared use classification and the adherence to
PA6.6 with 75% recycled cleaning and maintenance instructions.
Yarn type -
content A minimum service life of 10 years can be assumed,
Colouration solution-dyed yarn technical service life can be considerably longer.
PET with 88 % recycled
Primary
content
CQuest Bio backing,
Secondary backing heavy backing with textile -
bottom
Total pile weight 1000 g/m²
Total carpet weight 4420 g/m2
LCA: Calculation rules
Declared Unit System boundary
Type of EPD: Cradle-to-grave
Name Value Unit
Declared unit 1 m2 System boundaries of modules A, B, C, D:
Conversion factor to 1 kg 4.42 - Modules C3, C4 and D are indicated separately for
Grammage 4.42 kg/m2 three end-of-life scenarios:
Layer thickness 0.094 m - 1 landfill disposal
Mass reference 4.42 kg/m² - 2 municipal waste incineration
The declared unit refers to 1 m2 produced textile floor - 3 recovery in a cement plant
covering. The output of module A5 'Assembly' is 1 m2
installed textile floor covering. A1-A3 Production:
Energy supply and production of the basic material,
processing of secondary material, auxiliary material,
3 Environmental Product Declaration Interface – Tufted modular carpet tiles with CQuest Bio backing and a pile material of
PA 6.6 with 75% recycled content
transport of the material to the manufacturing site,
emissions, waste water treatment, packaging material C2 Transport:
and waste processing up to the landfill disposal of Transport of the carpet waste to a landfill, to the
residual waste (except radioactive waste). Benefits for municipal waste incineration plant (MWI) or to the
generated electricity and steam due to the incineration waste collection facility for recycling.
of production waste are aggregated.
Biogenic carbon that is stored in renewable material C3 Waste processing:
(wood resin, renewable additives, packaging paper) is C3-1: Landfill disposal needs no waste processing.
taken into account as well as the associated carbon C3-2: The impact from waste incineration (plant with
dioxide uptake from the air from which this biogenic R1>0.6), generated electricity and steam are listed in
carbon comes. the result table as exported energy. The biogenic
carbon that is stored in the renewable materials of the
A4 Transport: floor covering is released into the air as carbon dioxide
Transport of the packed textile floor covering emissions.
from factory gate to the place of installation. C3-3: Collection of the carpet waste for recovery in the
cement industry, waste processing (granulating),
A5 Installation: transport to the cement plant, emissions from the
Installation of the textile floor covering, processing of incineration. The biogenic carbon that is stored in the
installation waste and packaging waste up to the renewable materials of the floor covering is released
landfill disposal of residual waste (except radioactive into the air as carbon dioxide emissions.
waste), the production of the amount of carpet that
occurs as installation waste including its transport to C4 Disposal
the place of installation. C4-1: Impact from landfill disposal. The biogenic
Generated electricity and steam due to the incineration carbon that is stored in the renewable materials of the
of waste are listed in the result table as exported floor covering is released into the air as carbon dioxide
energy. emissions.
Biogenic carbon that is stored in renewable materials C4-2: The carpet waste leaves the system in
in installation waste and packaging paper is released module C3-2.
as carbon dioxide emissions into the air at the end of C4-3: The pre-processed carpet waste leaves the
life in module A5. system in module C3-3.
Preparation of the floor and auxiliary materials
(adhesives, fixing agents, PET connectors) are beyond D Recycling potential:
the system boundaries and not taken into account. Calculated benefits result from materials exclusive
secondary materials (net materials).
B1 Use:
Indoor emissions during the use stage. After the first D-A5: Benefits for generated energy due
year, no product- related Volatile Organic Compound to incineration of packaging and installation waste
(VOC) emissions are relevant due to known VOC (incineration plant with R1 > 0.6),
decay curves of the product. D-1: Benefits for generated energy due to landfill
disposal of carpet waste at the end-of-life,
B2 Maintenance: D-2: Benefits for generated energy due to incineration
Cleaning of the textile floor covering for a period of 1 of carpet waste at the end-of-life (incineration plant
year: with R1 > 0.6),
Vacuum cleaning – electricity supply D-3: Benefits for saved fossil energy and saved
Wet cleaning – electricity, water consumption, inorganic material due to recovery of the carpet in a
production of the cleaning agent, waste water cement plant.
treatment.
The declared values in this module have to be Comparability
multiplied by the assumed service life of the floor Basically, a comparison or an evaluation of EPD data
covering in the building in question. is only possible if all the data sets to be compared
were created according to EN 15804 and the building
B3 - B7: context, respectively the product-specific
The modules are not relevant and therefore not characteristics of performance, are taken into account.
declared.
Background data are taken from the GaBi database
C1 De-construction: 2020, service pack 40. Remaining data gaps are
The floor covering is de-constructed manually and no covered by the ecoinvent 3.6 database 2019.
additional environmental impact is caused.
LCA: Scenarios and additional technical information
The following information refer to the declared modules Transport to the construction site (A4)
and are the basis for calculations or can be used for Name Value Unit
further calculations. The indicated values refer to the Litres of fuel (truck, EURO 0-6
0.0103 l/100km
declared functional unit of all products with a total pile mix)
weight up to 1000 g/m2. Transport distance 700 km
Capacity utilisation (including
55 %
empty runs)
4 Environmental Product Declaration Interface – Tufted modular carpet tiles with CQuest Bio backing and a pile material of
PA 6.6 with 75% recycled content
Reuse, recovery and/or recycling potentials (D),
Installation in the building (A5) relevant scenario information
Name Value Unit Recovery or recycling potentials due to the three end-
Material loss 0.13 kg of-life scenarios (module C) are indicated separately.
Polyethene packaging waste and installation waste are
considered to be incinerated in a municipal waste Recycling in the cement industry (scenario 3)
incineration plant. Cardboard packaging waste is going VDZ e.V.
to be recycled. The organic material of the carpet is used as
Preparation of the floor and auxiliaries (adhesives, alternative fuel in a cement kiln. It mainly substitutes
fixing agents, PET connectors, etc.) are not taken into for lignite (64.5%), hard coal (26.5%) and petrol coke
account. (9.0%).
The inorganic material is substantially integrated into
the cement clinker and substitutes for original material
input.
Maintenance (B2)
The values for cleaning refer to 1 m2 floor covering
used in commercial areas per year. Depending on the
application based on ISO 10874, the technical service
life recommended by the manufacturer and the
anticipated strain on the floor by customers, the case-
specific useful life can be established. Based on this
useful life the effects of Module B2 need to be
calculated in order to obtain the overall environmental
impacts.
Name Value Unit
Maintenance cycle (wet cleaning) 1.5 1/year
Maintenance cycle (vacuum
208 1/year
cleaning)
Water consumption (wet cleaning) 0.004 m3
Cleaning agent (wet cleaning) 0.09 kg
Electricity consumption 0.314 kWh
Further information on cleaning and maintenance see
www.interface.com
End of Life (C1-C4)
Three different end-of-life scenarios are declared and
the results are indicated separately in module C.
Each scenario is calculated as a 100% scenario.
Scenario 1: 100% landfill disposal
Scenario 2: 100% municipal waste incineration (MWI)
with R1>0.6
Scenario 3: 100% recycling in the cement industry
If combinations of these scenarios have to be
calculated this should be done according to the
following scheme:
EOL-impact = x% impact (Scenario 1)
+ y% impact (Scenario 2)
+ z% impact (Scenario 3)
with x% + y% + z% = 100%
Name Value Unit
Collected as mixed construction
4.42 kg
waste (scenario 1 and 2)
Collected separately (scenario 3) 4.42 kg
Landfilling (scenario 1) 4.42 kg
Energy recovery (scenario 2) 4.42 kg
Energy recovery (scenario 3) 1.82 kg
Recycling (scenario 3) 2.6 kg
5 Environmental Product Declaration Interface – Tufted modular carpet tiles with CQuest Bio backing and a pile material of
PA 6.6 with 75% recycled content
LCA: Results
The LCA results refer to all declared products with a maximum total pile weight of 1000 g/m2. LCA results for
products with a maximum total pile weight of 600 g/m2 can be taken from the corresponding tables of the annexe.
Results for specific products with any other total pile weight can be calculated by using equation 1 given in the
annexe (see annexe chapter: 'General Information on the annexe').
The declared result figures in module B2 have to be multiplied by the assumed service life (in years) of the floor
covering in the building under consideration.
Information on un-declared modules: Modules B6, B7, C1, C3/1, C4/2 and C4/3 cause no additional impact (see
chapter "LCA: Calculation rules" in this document) and are not relevant. They are marked as 'modules not
declared' (MND). Module C2 represents the transport for scenarios 1, 2 and 3. Column D represents module
D/A5. The calculations are based on the CML characterization factors (version January 2016).
DESCRIPTION OF THE SYSTEM BOUNDARY (X = INCLUDED IN LCA; MND = MODULE NOT DECLARED;
MNR = MODULE NOT RELEVANT)
BENEFITS AND
CONSTRUCTI LOADS
PRODUCT STAGE ON PROCESS USE STAGE END OF LIFE STAGE BEYOND THE
STAGE SYSTEM
BOUNDARIES
6 Environmental Product Declaration Interface – Tufted modular carpet tiles with CQuest Bio backing and a pile material of
PA 6.6 with 75% recycled content
lairetam
waR
ylppus tropsnarT
gnirutcafunaM
eht
morf
tropsnarT
etis
eht
ot
etag
ylbmessA esU
ecnanetniaM
riapeR
tnemecalpeR tnemhsibrufeR
ygrene
lanoitarepO esu
retaw
lanoitarepO esu
noitcurtsnoc-eD
noitilomed tropsnarT
gnissecorp
etsaW
lasopsiD -esueR -yrevoceR -gnilcyceR laitnetop
A1 A2 A3 A4 A5 B1 B2 B3 B4 B5 B6 B7 C1 C2 C3 C4 D
X X X X X X X MNR MNR MNR MND MND MND X X X X
RESULTS OF THE LCA - ENVIRONMENTAL IMPACT according to EN 15804+A1: 1 m² floorcovering
Parameter Unit A1-A3 A4 A5 B1 B2 C2 C3/2 C3/3 C4/1 D D/1 D/2 D/3
GWP [kg CO2-Eq.] 6.51E+0 2.63E-1 4.21E-1 0.00E+0 2.92E-1 1.46E-2 5.67E+0 5.73E+0 1.20E+0 -2.52E-2 0.00E+0 -5.12E-1 -2.55E-1
-3.56E- -7.17E- -1.32E-
ODP [kg CFC11-Eq.] 2.44E-8 4.33E-177.33E-100.00E+0 1.21E-8 2.40E-182.01E-152.74E-159.66E-16 0.00E+0
16 15 15
AP [kg SO2-Eq.] 1.68E-2 1.11E-3 6.44E-4 0.00E+0 1.16E-3 6.17E-5 3.47E-3 3.68E-3 8.08E-4 -3.17E-5 0.00E+0 -6.42E-4 -9.44E-4
EP [kg (PO4)3--Eq.] 1.08E-2 2.79E-4 3.58E-4 0.00E+0 3.17E-4 1.55E-5 8.59E-4 9.03E-4 8.45E-4 -3.95E-6 0.00E+0 -8.00E-5 -1.17E-4
POCP [kg ethene-Eq.] 1.37E-3 -4.68E-4 3.25E-5 6.29E-5 1.48E-4 -2.60E-5 2.12E-4 1.50E-4 9.13E-5 -2.89E-6 0.00E+0 -5.86E-5 -9.12E-5
ADPE [kg Sb-Eq.] 1.34E-5 2.23E-8 4.07E-7 0.00E+0 4.43E-6 1.24E-9 1.95E-7 2.06E-7 5.77E-8 -4.70E-9 0.00E+0 -9.50E-8 -1.42E-7
ADPF [MJ] 1.23E+2 3.59E+0 3.88E+0 0.00E+0 6.76E+0 1.99E-1 2.95E+0 3.71E+0 4.45E+0 -3.53E-1 0.00E+0-7.18E+0-2.80E+1
GWP = Global warming potential; ODP = Depletion potential of the stratospheric ozone layer; AP = Acidification potential of land and water; EP =
Caption Eutrophication potential; POCP = Formation potential of tropospheric ozone photochemical oxidants; ADPE = Abiotic depletion potential for non-
fossil resources; ADPF = Abiotic depletion potential for fossil resources
RESULTS OF THE LCA - INDICATORS TO DESCRIBE RESOURCE USE according to EN 15804+A1: 1 m²
floorcovering
Parameter Unit A1-A3 A4 A5 B1 B2 C2 C3/2 C3/3 C4/1 D D/1 D/2 D/3
PERE [MJ] 3.16E+1 2.02E-1 1.72E+0 0.00E+0 1.20E+0 1.12E-2 1.38E+1 1.40E+1 3.22E-1 -9.47E-2 0.00E+0 -1.91E+0 -3.13E-1
PERM [MJ] 1.36E+1 0.00E+0 -3.39E-1 0.00E+0 0.00E+0 0.00E+0 -1.33E+1 -1.33E+1 0.00E+0 0.00E+0 0.00E+0 0.00E+0 0.00E+0
PERT [MJ] 4.52E+1 2.02E-1 1.38E+0 0.00E+0 1.20E+0 1.12E-2 4.78E-1 6.99E-1 3.22E-1 -9.47E-2 0.00E+0 -1.91E+0 -3.13E-1
PENRE [MJ] 1.18E+2 3.60E+0 4.55E+0 0.00E+0 7.86E+0 2.00E-1 2.04E+1 2.13E+1 4.59E+0 -4.35E-1 0.00E+0 -8.82E+0 -2.82E+1
PENRM [MJ] 1.74E+1 0.00E+0 -2.69E-1 0.00E+0 0.00E+0 0.00E+0 -1.71E+1 -1.71E+1 0.00E+0 0.00E+0 0.00E+0 0.00E+0 0.00E+0
PENRT [MJ] 1.35E+2 3.60E+0 4.28E+0 0.00E+0 7.86E+0 2.00E-1 3.24E+0 4.18E+0 4.59E+0 -4.35E-1 0.00E+0 -8.82E+0 -2.82E+1
SM [kg] 3.37E+0 0.00E+0 1.01E-1 0.00E+0 0.00E+0 0.00E+0 0.00E+0 0.00E+0 0.00E+0 0.00E+0 0.00E+0 0.00E+0 1.90E-1
RSF [MJ] 0.00E+0 0.00E+0 0.00E+0 0.00E+0 0.00E+0 0.00E+0 0.00E+0 0.00E+0 0.00E+0 0.00E+0 0.00E+0 0.00E+0 0.00E+0
NRSF [MJ] 0.00E+0 0.00E+0 0.00E+0 0.00E+0 0.00E+0 0.00E+0 0.00E+0 0.00E+0 0.00E+0 0.00E+0 0.00E+0 0.00E+0 0.00E+0
FW [m³] 3.38E-1 2.34E-4 1.07E-2 0.00E+0 4.27E-3 1.30E-5 1.62E-2 1.65E-2 5.63E-5 -1.10E-4 0.00E+0 -2.21E-3 -2.50E-3
PERE = Use of renewable primary energy excluding renewable primary energy resources used as raw materials; PERM = Use of
renewable primary energy resources used as raw materials; PERT = Total use of renewable primary energy resources; PENRE = Use of
non-renewable primary energy excluding non-renewable primary energy resources used as raw materials; PENRM = Use of non-
Caption
renewable primary energy resources used as raw materials; PENRT = Total use of non-renewable primary energy resources; SM = Use
of secondary material; RSF = Use of renewable secondary fuels; NRSF = Use of non-renewable secondary fuels; FW = Use of net fresh
water
RESULTS OF THE LCA – WASTE CATEGORIES AND OUTPUT FLOWS according to EN 15804+A1:
1 m² floorcovering
Parameter Unit A1-A3 A4 A5 B1 B2 C2 C3/2 C3/3 C4/1 D D/1 D/2 D/3
HWD [kg] 4.16E-7 1.68E-7 1.84E-8 0.00E+0 9.63E-10 9.30E-9 1.65E-8 3.99E-8 1.67E-8 -1.73E-10 0.00E+0 -3.52E-9 -6.47E-9
NHWD [kg] 3.47E-1 5.51E-4 4.94E-2 0.00E+0 5.63E-3 3.06E-5 1.30E+0 1.30E+0 4.40E+0 -2.01E-4 0.00E+0 -4.06E-3 -1.16E-1
RWD [kg] 4.84E-3 4.45E-6 1.49E-4 0.00E+0 3.38E-4 2.47E-7 1.18E-4 1.84E-4 5.53E-5 -3.23E-5 0.00E+0 -6.52E-4 -8.06E-5
CRU [kg] 0.00E+0 0.00E+0 0.00E+0 0.00E+0 0.00E+0 0.00E+0 0.00E+0 0.00E+0 0.00E+0 0.00E+0 0.00E+0 0.00E+0 0.00E+0
MFR [kg] 0.00E+0 0.00E+0 1.21E-1 0.00E+0 0.00E+0 0.00E+0 0.00E+0 1.44E+0 0.00E+0 0.00E+0 0.00E+0 0.00E+0 0.00E+0
MER [kg] 0.00E+0 0.00E+0 0.00E+0 0.00E+0 0.00E+0 0.00E+0 0.00E+0 0.00E+0 0.00E+0 0.00E+0 0.00E+0 0.00E+0 0.00E+0
EEE [MJ] 0.00E+0 0.00E+0 2.07E-1 0.00E+0 0.00E+0 0.00E+0 5.49E+0 0.00E+0 0.00E+0 0.00E+0 0.00E+0 0.00E+0 0.00E+0
EET [MJ] 0.00E+0 0.00E+0 3.88E-1 0.00E+0 0.00E+0 0.00E+0 1.04E+1 6.33E+1 0.00E+0 0.00E+0 0.00E+0 0.00E+0 0.00E+0
HWD = Hazardous waste disposed; NHWD = Non-hazardous waste disposed; RWD = Radioactive waste disposed; CRU = Components
Caption for re-use; MFR = Materials for recycling; MER = Materials for energy recovery; EEE = Exported electrical energy; EEE = Exported
thermal energy
Information on the biogenic carbon content:
The textile floor covering contains renewable materials with stored biogenic carbon. During the growth phase of
plants carbon dioxide (CO ) is absorbed and transformed into stored biogenic carbon.
2
This amount of CO uptake is taken into account in module A1-A3 as a negative value that reduces the total
2
amount of the GWP. At the end of life the same amount of CO is released into the air as emissions. These CO
2 2
emissions increase the amount of the GWP in the three scenarios landfill disposal, municipal incineration and
recovery in the cement industry.
Biogenic carbon content per m2 textile floor covering: 0.27 kg C
Corresponding carbon dioxide uptake/emissions: 0.99 kg CO
2
Not all of the life cycle inventories applied in this study support the methodological approach for the waste and
water indicators. The data are based on publications of industry. The indicators for waste and water of the system
are evaluated but contain a higher degree of uncertainty.
References
EN 1307 ECHA candidate list
DIN EN 1307: 2014+A1:2016: Textile floor coverings - Candidate List of substances of very high concern
Classification (SVHCs) for authorisation, 16.01.2020, European
EN 13501-1 Chemicals Agency (ECHA), Helsinki, Finland
DIN EN 13501-1:2010-01: Fire classification of ecoinvent 3.6
construction products and building elements - Part 1: ecoinvent, Zurich, Switzerland, database version 3.6,
Classification using data from reaction to fire tests published September 2019
EN 14041 GaBi database 2020
DIN EN 14041: 2018-05: Resilient, textile and laminate GaBi Software-System and Database for Life Cycle
floor coverings - Essential characteristics Engineering, thinkstep AG, Leinfelden-Echterdingen,
EN 15804 service pack 40, 2020
EN 15804:2012-04+A1 2013/, Sustainability of IBU 2016
construction works — Environmental Product IBU (2016): General Programme Instructions for the
Declarations — Core rules for the product category of Preparation of EPDs at the Institut Bauen und Umwelt
construction products e.V., Version 1.1 Institut Bauen und Umwelt e.V.,
EN 16810 Berlin, www.ibu-epd.de
DIN EN 16810: 2017-08: Resilient, textile and laminate PCR Part A
floor coverings – Environmental product declarations – Product Category Rules for Construction Products
Product category rules from the range of Environmental Product Declarations.
ISO 10874 Part A: Calculation Rules for the Life Cycle
DIN EN ISO 10874: 2012-04: Resilient, textile and Assessment and Requirements on the Background
laminate floor coverings - Classification Report, V1.8, Berlin: Institut Bauen und Umwelt e.V.
ISO 14025 (IBU), July 2019
DIN EN /ISO 14025:2011-10: Environmental labels PCR Part B
and declarations — Type III environmental Product Category Rules for Construction Products
declarations — Principles and procedures from the range of Environmental Product Declarations
ISO 15686 of Institut Bauen und Umwelt (IBU),
ISO 15686: Buildings and constructed assets - Part B: Requirements on the EPD for floor coverings,
Service life planning V1.2, Berlin: Institut Bauen und Umwelt e.V. (IBU),
ISO 15686-1: 2011-05: Part 1: General principles and February 2018
framework PRODIS
ISO 15686-2: 2012-05: Part 2: Service life prediction Product Information System (PRODIS) of the
procedures European Carpet Industry, Gemeinschaft
ISO 15686-7: 2006-03: Part 7: Performance umweltfreundlicher Teppichboden e.V (GUT) and
evaluation for feedback of service life data European Carpet and Rug Association
from practice (ECRA), http://www.pro-dis.info
ISO 15686-8: 2008-06: Part 8: Reference service life REACH
and service-life estimation Regulation (EC) No 1907/2006 of the European
Regulation (EU) No. 305/2011 Parliament and of the Council of 18 December 2006
Regulation No. 305/2011 Construction Products concerning the Registration, Evaluation, Authorisation
Regulation (CPR) of the European Council and of the and Restriction of Chemicals (REACH). Last update:
European Parliament, April 2011 25.03.2014 (Status: 27.06.2018)
CML characterization factors VDZ e.V.
Impact assessment characterization factors, Institute of Association of German Cement Works, Ed. Environ-
Environmental Sciences - in Dutch 'Centrum voor mental Data of the German Cement Industry 2018
Milieuwetenschappen in Leiden' (CML), Leiden, The
Netherlands
7 Environmental Product Declaration Interface – Tufted modular carpet tiles with CQuest Bio backing and a pile material of
PA 6.6 with 75% recycled content
Publisher
Institut Bauen und Umwelt e.V. Tel +49 (0)30 3087748- 0
Panoramastr. 1 Fax +49 (0)30 3087748- 29
10178 Berlin Mail info@ibu-epd.com
Germany Web www.ibu-epd.com
Programme holder
Institut Bauen und Umwelt e.V. Tel +49 (0)30 - 3087748- 0
Panoramastr 1 Fax +49 (0)30 – 3087748 - 29
10178 Berlin Mail info@ibu-epd.com
Germany Web www.ibu-epd.com
Author of the Life Cycle
Assessment Tel +49 (0)241 96843 410
Gemeinschaft umweltfreundlicher Fax +49 (0)241 96843 400
Teppichboden (GUT) e.V. Mail mail@gut-ev.de
Schönebergstraße 2 Web www.gut-ev.org
52068 Aachen
Germany
Owner of the Declaration
Interface Europe Manufacturing Tel +31 33 277 55 55
BV Fax +31 33 277 55 54
Industrielaan 15 Mail receptie@interface.com
3925ZG Scherpenzeel Web www.interface.com
Netherlands
