ENVIRONMENTAL PRODUCT DECLARATION
as per ISO 14025 and EN 15804+A1
Owner of the Declaration Interface Europe Manufacturing BV
Programme holder Institut Bauen und Umwelt e.V. (IBU)
Publisher Institut Bauen und Umwelt e.V. (IBU)
Declaration number EPD-INT-20200182-CCC1-EN
Issue date 05.11.2020
Valid to 04.11.2025
Modular carpet tiles with CQuest Bio backing
pile material solution-dyed polyamide 6,
maximum total pile weight 900 g/m2
Interface®
www.ibu-epd.com | https://epd-online.com
Umwelt Produktdeklaration Name des Herstellers – Name des Produkts
General Information
Interface® Modular carpet tiles with CQuest
Bio backing
pile material solution-dyed PA 6,
maximum total pile weight 900 g/m2
Programme holder Owner of the declaration
IBU – Institut Bauen und Umwelt e.V. Interface Europe Manufacturing BV
Panoramastr. 1 Industrielaan 15
10178 Berlin 3925 ZG Scherpenzeel
Germany The Netherlands
Declaration number Declared product / declared unit
EPD-INT-20200182-CCC1-EN 1 m² tufted modular carpet tiles with CQuest Bio
backing (CQB) and a pile material of PA 6
This declaration is based on the product Scope:
category rules: The manufacturer declaration applies to modular
Floor coverings, 02/2018 carpet tiles with CQuest Bio backing and a maximum
(PCR checked and approved by the SVR) total pile material of 900 g/m2 PA 6. The products are
tufted in Scherpenzeel, The Netherlands, or in
Craigavon, Ireland. They are back coated in
Issue date
Scherpenzeel.
05.11.2020
LCA results for products with a maximum total pile
weight of 400 g/m2 can be taken from the
Valid to
corresponding tables of the annexe. Specific data for
04.11.2025 every product within the declared group of products in
relation to its total pile weight can be calculated by
using equation 1 given in the annexe (see annexe
chapter: 'General Information on the annexe').
The declaration is only valid in conjunction with a valid
GUT-PRODIS license of the product.
The owner of the declaration shall be liable for the
underlying information and evidence; the IBU shall not
be liable with respect to manufacturer information, life
cycle assessment data and evidences.
The EPD was created according to the specifications
of EN 15804+A1. In the following, the standard will be
simplified as EN 15804.
Verification
The standard EN 15804 serves as the core PCR
Independent verification of the declaration and data
according to ISO 14025:2010
Dipl. Ing. Hans Peters internally x externally
(chairman of Institut Bauen und Umwelt e.V.)
Dr. Alexander Röder Dr. Frank Werner
(Managing Director Institut Bauen und Umwelt e.V.)) (Independent verifier)
Product
Information about the enterprise way that is restorative to the planet and creates a
Interface, Inc. is a global flooring company specializing climate fit for life.
in carbon-neutral carpet tile and resilient flooring,
including luxury vinyl tile (LVT) and nora® rubber Product description/Product definition
flooring. We help our customers create high- Tufted modular carpet tiles having a surface pile of
performance interior spaces that support well-being, solution-dyed polyamide 6 and a CQuest Bio backing
productivity, and creativity, as well as the sustainability system.
of the planet. Our mission, Climate Take Back™, CQuest Bio backing system: Backing compound based
invites you to join us as we commit to operating in a on wood resin, containing a recycled filler, glass-fleece
reinforcement and polypropylene covering fleece.
2 Environmental Product Declaration Interface – Tufted modular carpet tiles with CQuest Bio backing and a pile material of
PA 6
The minimum recycled content out of total weight is
60% with a total pile weight of 900 g/m2. Performance data of the product in accordance with
The declaration applies to a group of products with a the declaration of performance with respect to its
maximum total pile weight of 900 g/m2. essential characteristics according to EN 14041.
LCA results for products with a maximum total pile Additional product properties in accordance with EN
weight of 400 g/m2 can be taken from the 1307 can be found on the Product Information System
corresponding tables of the annexe. PRODIS using the PRODIS registration number of the
Results for specific products with any other total pile product (www.pro-dis.info) or on the manufacturer's
weight can be calculated by using equation 1 given in technical information section (www.interface.com).
the annexe (see annexe chapter: 'General Information
on the annexe'). Base materials/Ancillary materials
For the placing on the market of the product in the
European Union/European Free Trade Association Name Value Unit
(EU/EFTA) (with the exception of Switzerland) Polyamide 6 20.5 %
Regulation (EU) No. 305/2011 Construction Product Polyester 2.7 %
Regulation (CPR) applies. The product needs a Polypropylene 1.1 %
Declaration of Performance (DoP) taking into Limestone 53.8 %
consideration EN 14041 and the CE-marking. The DoP Aluminum hydroxide 5.8 %
of the product can be found on the manufacturer's Ethylene vinyl acetate (EVA) 6.6 %
technical information section. For the application and Wood resin 6.6 %
use of the product the respective national provisions
Glass fibre 0.8 %
apply.
Additives 2.1 %
Application
The products are registered in the GUT-PRODIS
According to the use class as defined in EN 1307 the
Information System. The PRODIS system ensures the
products can be used in all professional areas which
compliance with limitations of various chemicals and
require class 33 or less.
Volatile Organic Compound (VOC)-emissions and a
ban on the use of all substances that are listed as
'Substances of Very High Concern' (SVHC) under
REACH.
This product contains substances listed in the ECHA
Technical Data candidate list (27.06.2018) exceeding 0.1 percentage
The performance data listed in the DoP apply. by mass: no
Name Value Unit
Modular carpet tiles, Reference service life
Product Form -
50 cm x 50 cm A calculation of the reference service life according to
Type of manufacture tufted carpet - ISO 15686 is not possible.
Yarn type PA 6 - The service life of textile floor coverings strongly
Colouration solution-dyed yarn depends on the correct installation taking into account
PET with 88 % recycled the declared use classification and the adherence to
Primary
content cleaning and maintenance instructions.
CQuest Bio backing, A minimum service life of 10 years can be assumed,
Secondary backing heavy backing with textile - technical service life can be considerably longer.
bottom
Total pile weight 900 g/m²
Total carpet weight 4390 g/m2
LCA: Calculation rules
Declared Unit System boundaries of modules A, B, C, D:
Modules C3, C4 and D are indicated separately for
three end-of-life scenarios:
Name Value Unit - 1 landfill disposal
Declared unit 1 m2 - 2 municipal waste incineration
Conversion factor to 1 kg 4.39 - - 3 recovery in a cement plant
Mass reference 4.39 kg/m²
The declared unit refers to 1 m2 produced textile floor A1-A3 Production:
covering. The output of module A5 'Assembly' is 1 m2 Energy supply and production of the basic material,
installed textile floor covering. processing of secondary material, auxiliary material,
transport of the material to the manufacturing site,
emissions, waste water treatment, packaging material
System boundary and waste processing up to the landfill disposal of
residual waste (except radioactive waste). Benefits for
Type of EPD: Cradle-to-grave generated electricity and steam due to the incineration
of production waste are aggregated.
Biogenic carbon that is stored in renewable material
3 Environmental Product Declaration Interface – Tufted modular carpet tiles with CQuest Bio backing and a pile material of
PA 6
(wood resin, renewable additives, packaging paper) is
taken into account as well as the associated carbon C3 Waste processing:
dioxide uptake from the air from which this biogenic C3-1: Landfill disposal needs no waste processing.
carbon comes. C3-2: The impact from waste incineration (plant with
R1>0.6), generated electricity and steam are listed in
A4 Transport: the result table as exported energy. The biogenic
Transport of the packed textile floor covering carbon that is stored in the renewable materials of the
from factory gate to the place of installation. floor covering is released into the air as carbon dioxide
emissions.
A5 Installation: C3-3: Collection of the carpet waste for recovery in the
Installation of the textile floor covering, processing of cement industry, waste processing (granulating),
installation waste and packaging waste up to the transport to the cement plant, emissions from the
landfill disposal of residual waste (except radioactive incineration. The biogenic carbon that is stored in the
waste), the production of the amount of carpet that renewable materials of the floor covering is released
occurs as installation waste including its transport to into the air as carbon dioxide emissions.
the place of installation. Generated electricity and
steam due to the incineration of waste are listed in the C4 Disposal
result table as exported energy. C4-1: Impact from landfill disposal. The biogenic
Biogenic carbon that is stored in renewable materials carbon that is stored in the renewable materials of the
in installation waste and packaging paper is released floor covering is released into the air as carbon dioxide
as carbon dioxide emissions into the air at the end of emissions.
life in module A5. C4-2: The carpet waste leaves the system in
Preparation of the floor and auxiliary materials module C3-2.
(adhesives, fixing agents, PET connectors) are beyond C4-3: The pre-processed carpet waste leaves the
the system boundaries and not taken into account. system in module C3-3.
B1 Use: D Recycling potential:
Indoor emissions during the use stage. After the first Calculated benefits result from materials exclusive
year, no product- related Volatile Organic Compound secondary materials (net materials).
(VOC) emissions are relevant due to known VOC
decay curves of the product. D-A5: Benefits for generated energy due
to incineration of packaging and installation waste
B2 Maintenance: (incineration plant with R1 > 0.6),
Cleaning of the textile floor covering for a period of 1 D-1: Benefits for generated energy due to landfill
year: disposal of carpet waste at the end-of-life,
Vacuum cleaning – electricity supply. D-2: Benefits for generated energy due to incineration
Wet cleaning – electricity, water consumption, of carpet waste at the end-of-life (incineration plant
production of the cleaning agent, waste water with R1 > 0.6),
treatment. D-3: Benefits for saved fossil energy and saved
The declared values in this module have to be inorganic material due to recovery of the carpet in a
multiplied by the assumed service life of the floor cement plant.
covering in the building in question.
Comparability
B3 - B7: Basically, a comparison or an evaluation of EPD data
The modules are not relevant and therefore not is only possible if all the data sets to be compared
declared. were created according to EN 15804 and the building
context, respectively the product-specific
C1 De-construction: characteristics of performance, are taken into account.
The floor covering is de-constructed manually and no
additional environmental impact is caused. Background data are taken from the GaBi database
2020, service pack 40. Remaining data gaps are
C2 Transport: covered by the ecoinvent 3.6 database 2019.
Transport of the carpet waste to a landfill, to the
municipal waste incineration plant (MWI) or to the
waste collection facility for recycling.
LCA: Scenarios and additional technical information
The following information refer to the declared modules
and are the basis for calculations or can be used for Installation in the building (A5)
further calculations. The indicated values refer to the Name Value Unit
declared functional unit of all products with a total pile Material loss 0.13 kg
weight up to 900 g/m2. Polyethene packaging waste and installation waste are
considered to be incinerated in a municipal waste
Transport to the construction site (A4) incineration plant. Cardboard packaging waste is going
Name Value Unit to be recycled.
Litres of fuel (truck, EURO 0-6 mix) 0.0103 l/100km Preparation of the floor and auxiliaries (adhesives,
Transport distance 700 km fixing agents, PET connectors, etc.) are not taken into
Capacity utilisation (including empty account.
55 %
runs)
4 Environmental Product Declaration Interface – Tufted modular carpet tiles with CQuest Bio backing and a pile material of
PA 6
Maintenance (B2)
The values for cleaning refer to 1 m2 floor covering
used in commercial areas per year. Depending on the
application based on ISO 10874, the technical service
life recommended by the manufacturer and the
anticipated strain on the floor by customers, the case-
specific useful life can be established. Based on this
useful life the effects of Module B2 need to be
calculated in order to obtain the overall environmental
impacts.
Name Value Unit
Maintenance cycle (wet cleaning) 1.5 1/year
Maintenance cycle (vacuum cleaning) 208 1/year
Water consumption (wet cleaning) 0.004 m3
Cleaning agent (wet cleaning) 0.09 kg
Electricity consumption 0.314 kWh
Further information on cleaning and maintenance see
www.interface.com
End of Life (C1-C4)
Three different end-of-life scenarios are declared and
the results are indicated separately in module C.
Each scenario is calculated as a 100% scenario.
Scenario 1: 100% landfill disposal
Scenario 2: 100% municipal waste incineration (MWI)
with R1>0.6
Scenario 3: 100% recycling in the cement industry
If combinations of these scenarios have to be
calculated this should be done according to the
following scheme:
EOL-impact = x% impact (Scenario 1)
+ y% impact (Scenario 2)
+ z% impact (Scenario 3)
with x% + y% + z% = 100%
Name Value Unit
Collected as mixed construction waste
4.39 kg
(scenario 1 and 2)
Collected separately (scenario 3) 4.39 kg
Landfilling (scenario 1) 4.39 kg
Energy recovery (scenario 2) 4.39 kg
Energy recovery (scenario 3) 1.74 kg
Recycling (scenario 3) 2.65 kg
Reuse, recovery and/or recycling potentials (D),
relevant scenario information
Recovery or recycling potentials due to the three end-
of-life scenarios (module C) are indicated separately.
Recycling in the cement industry (scenario 3)
VDZ e.V.
The organic material of the carpet is used as an
alternative fuel in a cement kiln. It mainly substitutes
for lignite (64.5%), hard coal (26.5%) and petrol coke
(9.0%).
The inorganic material is substantially integrated into
the cement clinker and substitutes for original material
input.
5 Environmental Product Declaration Interface – Tufted modular carpet tiles with CQuest Bio backing and a pile material of
PA 6
LCA: Results
The LCA results refer to all declared products with a maximum total pile weight of 900 g/m2.
LCA results for products with a maximum total pile weight of 400 g/m2 can be taken from the corresponding tables
of the annexe. Results for specific products with any other total pile weight can be calculated by using equation 1
given in the annexe (see annexe chapter: 'General Information on the annexe'). The declared result figures in
module B2 have to be multiplied by the assumed service life (in years) of the floor covering in the building under
consideration.
Information on un-declared modules: Modules B6, B7, C1, C3/1, C4/2 and C4/3 cause no additional impact (see
chapter "LCA: Calculation rules" in this document) and are not relevant. They are marked as 'modules not
declared' (MND). Module C2 represents the transport for scenarios 1, 2 and 3. Column D represents module
D/A5. The calculations are based on the CML characterization factors (version January 2016).
DESCRIPTION OF THE SYSTEM BOUNDARY (X = INCLUDED IN LCA; MND = MODULE NOT DECLARED;
MNR = MODULE NOT RELEVANT)
BENEFITS AND
CONSTRUCTI LOADS
PRODUCT STAGE ON PROCESS USE STAGE END OF LIFE STAGE BEYOND THE
STAGE SYSTEM
BOUNDARIES
6 Environmental Product Declaration Interface – Tufted modular carpet tiles with CQuest Bio backing and a pile material of
PA 6
lairetam
waR
ylppus tropsnarT
gnirutcafunaM
eht
morf
tropsnarT
etis
eht
ot
etag
ylbmessA esU
ecnanetniaM
riapeR
tnemecalpeR tnemhsibrufeR
ygrene
lanoitarepO esu
retaw
lanoitarepO esu
noitcurtsnoc-eD
noitilomed tropsnarT
gnissecorp
etsaW
lasopsiD -esueR -yrevoceR -gnilcyceR laitnetop
A1 A2 A3 A4 A5 B1 B2 B3 B4 B5 B6 B7 C1 C2 C3 C4 D
X X X X X X X MNR MNR MNR MND MND MND X X X X
RESULTS OF THE LCA - ENVIRONMENTAL IMPACT according to EN 15804+A1: 1 m² floorcovering
Parameter Unit A1-A3 A4 A5 B1 B2 C2 C3/2 C3/3 C4/1 D D/1 D/2 D/3
GWP [kg CO2-Eq.] 9.94E+0 2.62E-1 6.85E-1 0.00E+0 2.92E-1 1.45E-2 5.49E+0 5.55E+0 1.19E+0 -4.61E-2 0.00E+0-1.21E+0-3.83E-1
-6.52E- -1.71E- -1.80E-
ODP [kg CFC11-Eq.] 2.45E-8 4.30E-177.34E-100.00E+0 1.21E-8 2.39E-182.07E-152.79E-159.60E-16 0.00E+0
16 14 15
AP [kg SO2-Eq.] 2.03E-2 1.10E-3 7.44E-4 0.00E+0 1.16E-3 6.12E-5 3.24E-3 3.45E-3 8.03E-4 -5.81E-5 0.00E+0 -1.52E-3 -1.37E-3
EP [kg (PO4)3--Eq.] 1.08E-2 2.77E-4 3.57E-4 0.00E+0 3.17E-4 1.54E-5 7.97E-4 8.41E-4 8.39E-4 -7.24E-6 0.00E+0 -1.90E-4 -1.71E-4
POCP [kg ethene-Eq.] 2.66E-3 -4.65E-4 7.07E-5 6.29E-5 1.48E-4 -2.58E-5 1.99E-4 1.38E-4 9.06E-5 -5.30E-6 0.00E+0 -1.39E-4 -1.40E-4
ADPE [kg Sb-Eq.] 1.36E-5 2.21E-8 4.16E-7 0.00E+0 4.43E-6 1.23E-9 2.05E-7 2.16E-7 5.73E-8 -8.61E-9 0.00E+0 -2.25E-7 -1.62E-7
ADPF [MJ] 2.02E+2 3.56E+0 6.25E+0 0.00E+0 6.76E+0 1.98E-1 2.97E+0 3.73E+0 4.42E+0 -6.46E-1 0.00E+0-1.70E+1-4.69E+1
GWP = Global warming potential; ODP = Depletion potential of the stratospheric ozone layer; AP = Acidification potential of land and water; EP =
Caption Eutrophication potential; POCP = Formation potential of tropospheric ozone photochemical oxidants; ADPE = Abiotic depletion potential for non-
fossil resources; ADPF = Abiotic depletion potential for fossil resources
RESULTS OF THE LCA - INDICATORS TO DESCRIBE RESOURCE USE according to EN 15804+A1: 1 m²
floorcovering
Parameter Unit A1-A3 A4 A5 B1 B2 C2 C3/2 C3/3 C4/1 D D/1 D/2 D/3
PERE [MJ] 3.37E+1 2.01E-1 1.78E+0 0.00E+0 1.20E+0 1.12E-2 1.38E+1 1.40E+1 3.20E-1 -1.74E-1 0.00E+0 -4.54E+0 -4.32E-1
PERM [MJ] 1.36E+1 0.00E+0 -3.39E-1 0.00E+0 0.00E+0 0.00E+0 -1.33E+1 -1.33E+1 0.00E+0 0.00E+0 0.00E+0 0.00E+0 0.00E+0
PERT [MJ] 4.74E+1 2.01E-1 1.44E+0 0.00E+0 1.20E+0 1.12E-2 4.93E-1 7.12E-1 3.20E-1 -1.74E-1 0.00E+0 -4.54E+0 -4.32E-1
PENRE [MJ] 1.96E+2 3.58E+0 6.88E+0 0.00E+0 7.86E+0 1.99E-1 4.15E+1 4.24E+1 4.56E+0 -7.96E-1 0.00E+0 -2.09E+1 -4.72E+1
PENRM [MJ] 1.74E+1 0.00E+0 -2.69E-1 0.00E+0 0.00E+0 0.00E+0 -3.82E+1 -3.82E+1 0.00E+0 0.00E+0 0.00E+0 0.00E+0 0.00E+0
PENRT [MJ] 2.13E+2 3.58E+0 6.62E+0 0.00E+0 7.86E+0 1.99E-1 3.28E+0 4.21E+0 4.56E+0 -7.96E-1 0.00E+0 -2.09E+1 -4.72E+1
SM [kg] 2.64E+0 0.00E+0 7.92E-2 0.00E+0 0.00E+0 0.00E+0 0.00E+0 0.00E+0 0.00E+0 0.00E+0 0.00E+0 0.00E+0 2.00E-1
RSF [MJ] 0.00E+0 0.00E+0 0.00E+0 0.00E+0 0.00E+0 0.00E+0 0.00E+0 0.00E+0 0.00E+0 0.00E+0 0.00E+0 0.00E+0 0.00E+0
NRSF [MJ] 0.00E+0 0.00E+0 0.00E+0 0.00E+0 0.00E+0 0.00E+0 0.00E+0 0.00E+0 0.00E+0 0.00E+0 0.00E+0 0.00E+0 0.00E+0
FW [m³] 3.39E-1 2.33E-4 1.07E-2 0.00E+0 4.27E-3 1.29E-5 1.63E-2 1.66E-2 5.59E-5 -2.01E-4 0.00E+0 -5.26E-3 -4.05E-3
PERE = Use of renewable primary energy excluding renewable primary energy resources used as raw materials; PERM = Use of
renewable primary energy resources used as raw materials; PERT = Total use of renewable primary energy resources; PENRE = Use of
non-renewable primary energy excluding non-renewable primary energy resources used as raw materials; PENRM = Use of non-
Caption
renewable primary energy resources used as raw materials; PENRT = Total use of non-renewable primary energy resources; SM = Use
of secondary material; RSF = Use of renewable secondary fuels; NRSF = Use of non-renewable secondary fuels; FW = Use of net fresh
water
RESULTS OF THE LCA – WASTE CATEGORIES AND OUTPUT FLOWS according to EN 15804+A1:
1 m² floorcovering
Parameter Unit A1-A3 A4 A5 B1 B2 C2 C3/2 C3/3 C4/1 D D/1 D/2 D/3
HWD [kg] 4.27E-7 1.66E-7 1.87E-8 0.00E+0 9.63E-10 9.24E-9 1.76E-8 4.09E-8 1.66E-8 -3.17E-10 0.00E+0 -8.31E-9 -1.02E-8
NHWD [kg] 2.67E-1 5.47E-4 4.99E-2 0.00E+0 5.63E-3 3.04E-5 1.39E+0 1.39E+0 4.37E+0 -3.68E-4 0.00E+0 -9.62E-3 -1.23E-1
RWD [kg] 4.42E-3 4.43E-6 1.37E-4 0.00E+0 3.38E-4 2.46E-7 1.21E-4 1.87E-4 5.50E-5 -5.93E-5 0.00E+0 -1.55E-3 -1.11E-4
CRU [kg] 0.00E+0 0.00E+0 0.00E+0 0.00E+0 0.00E+0 0.00E+0 0.00E+0 0.00E+0 0.00E+0 0.00E+0 0.00E+0 0.00E+0 0.00E+0
MFR [kg] 0.00E+0 0.00E+0 1.21E-1 0.00E+0 0.00E+0 0.00E+0 0.00E+0 1.52E+0 0.00E+0 0.00E+0 0.00E+0 0.00E+0 0.00E+0
MER [kg] 0.00E+0 0.00E+0 0.00E+0 0.00E+0 0.00E+0 0.00E+0 0.00E+0 0.00E+0 0.00E+0 0.00E+0 0.00E+0 0.00E+0 0.00E+0
EEE [MJ] 0.00E+0 0.00E+0 1.92E-1 0.00E+0 0.00E+0 0.00E+0 4.98E+0 0.00E+0 0.00E+0 0.00E+0 0.00E+0 0.00E+0 0.00E+0
EET [MJ] 0.00E+0 0.00E+0 3.61E-1 0.00E+0 0.00E+0 0.00E+0 9.51E+0 6.08E+1 0.00E+0 0.00E+0 0.00E+0 0.00E+0 0.00E+0
HWD = Hazardous waste disposed; NHWD = Non-hazardous waste disposed; RWD = Radioactive waste disposed; CRU = Components
Caption for re-use; MFR = Materials for recycling; MER = Materials for energy recovery; EEE = Exported electrical energy; EEE = Exported
thermal energy
Information on the biogenic carbon content: The textile floor covering contains renewable materials with stored
biogenic carbon. During the growth phase of plants carbon dioxide (CO ) is absorbed and transformed into stored
2
biogenic carbon. This amount of CO uptake is taken into account in module A1-A3 as a negative value that
2
reduces the total amount of the GWP. At the end of life the same amount of CO is released into the air as
2
emissions. These CO emissions increase the amount of the GWP in the three scenarios landfill disposal,
2
municipal incineration and recovery in the cement industry.
Biogenic carbon content per m2 textile floor covering: 0.27 kg C
Corresponding carbon dioxide uptake/emissions: 0.99 kg CO
2
Not all of the life cycle inventories applied in this study support the methodological approach for the waste and
water indicators. The data are based on publications of industry. The indicators for waste and water of the system
are evaluated but contain a higher degree of uncertainty.
References
EN 1307 ECHA candidate list
DIN EN 1307: 2014+A1:2016: Textile floor coverings - Candidate List of substances of very high concern
Classification (SVHCs) for authorisation, 16.01.2020, European
EN 13501-1 Chemicals Agency (ECHA), Helsinki, Finland
DIN EN 13501-1:2010-01: Fire classification of ecoinvent 3.6
construction products and building elements - Part 1: ecoinvent, Zurich, Switzerland, database version 3.6,
Classification using data from reaction to fire tests published September 2019
EN 14041 GaBi database 2020
DIN EN 14041: 2018-05: Resilient, textile and laminate GaBi Software-System and Database for Life Cycle
floor coverings - Essential characteristics Engineering, thinkstep AG, Leinfelden-Echterdingen,
EN 15804 service pack 40, 2020
EN 15804:2012-04+A1 2013/, Sustainability of IBU 2016
construction works — Environmental Product IBU (2016): General Programme Instructions for the
Declarations — Core rules for the product category of Preparation of EPDs at the Institut Bauen und Umwelt
construction products e.V., Version 1.1 Institut Bauen und Umwelt e.V.,
EN 16810 Berlin, www.ibu-epd.de
DIN EN 16810: 2017-08: Resilient, textile and laminate PCR Part A
floor coverings – Environmental product declarations – Product Category Rules for Construction Products
Product category rules from the range of Environmental Product Declarations.
ISO 10874 Part A: Calculation Rules for the Life Cycle
DIN EN ISO 10874: 2012-04: Resilient, textile and Assessment and Requirements on the Background
laminate floor coverings - Classification Report, V1.8, Berlin: Institut Bauen und Umwelt e.V.
ISO 14025 (IBU), July 2019
DIN EN /ISO 14025:2011-10: Environmental labels PCR Part B
and declarations — Type III environmental Product Category Rules for Construction Products
declarations — Principles and procedures from the range of Environmental Product Declarations
ISO 15686 of Institut Bauen und Umwelt (IBU), Part B: Require-
ISO 15686: Buildings and constructed assets - ments on the EPD for floor coverings, V1.2, Berlin:
Service life planning Institut Bauen und Umwelt e.V. (IBU), February 2018
ISO 15686-1: 2011-05: Part 1: General principles and PRODIS
framework Product Information System (PRODIS) of the
ISO 15686-2: 2012-05: Part 2: Service life prediction European Carpet Industry, Gemeinschaft
procedures umweltfreundlicher Teppichboden e.V (GUT) and
ISO 15686-7: 2006-03: Part 7: Performance European Carpet and Rug Association
evaluation for feedback of service life data (ECRA), http://www.pro-dis.info
from practice REACH
ISO 15686-8: 2008-06: Part 8: Reference service life Regulation (EC) No 1907/2006 of the European
and service-life estimation Parliament and of the Council of 18 December 2006
Regulation (EU) No. 305/2011 concerning the Registration, Evaluation, Authorisation
Regulation No. 305/2011 Construction Products and Restriction of Chemicals (REACH). Last update:
Regulation (CPR) of the European Council and of the 25.03.2014 (Status: 27.06.2018)
European Parliament, April 2011 VDZ e.V.
CML characterization factors Association of German Cement Works, Ed. Environ-
Impact assessment characterization factors, Institute of mental Data of the German Cement Industry 2018
Environmental Sciences - in Dutch 'Centrum voor
Milieuwetenschappen in Leiden' (CML), Leiden, The
Netherlands
7 Environmental Product Declaration Interface – Tufted modular carpet tiles with CQuest Bio backing and a pile material of
PA 6
Publisher
Institut Bauen und Umwelt e.V. Tel +49 (0)30 3087748- 0
Panoramastr. 1 Fax +49 (0)30 3087748- 29
10178 Berlin Mail info@ibu-epd.com
Germany Web www.ibu-epd.com
Programme holder
Institut Bauen und Umwelt e.V. Tel +49 (0)30 - 3087748- 0
Panoramastr 1 Fax +49 (0)30 – 3087748 - 29
10178 Berlin Mail info@ibu-epd.com
Germany Web www.ibu-epd.com
Author of the Life Cycle
Assessment Tel +49 (0)241 96843 410
Gemeinschaft umweltfreundlicher Fax +49 (0)241 96843 400
Teppichboden (GUT) e.V. Mail mail@gut-ev.de
Schönebergstraße 2 Web www.gut-ev.org
52068 Aachen
Germany
Owner of the Declaration
Interface Europe Manufacturing Tel +31 33 277 55 55
BV Fax +31 33 277 55 54
Industrielaan 15 Mail receptie@interface.com
3925ZG Scherpenzeel Web www.interface.com
Netherlands
