Environmental product declaration
in accordance with ISO 14025 and EN 15804+A2
TVE-Q
Owner of the declaration: Program operator:
TROX Group The Norwegian EPD Foundation
Product: Declaration number:
TVE-Q
Registration number:
Declared unit:
1 pcs Issue date:
This declaration is based on Product Category Rules: Valid to:
CEN Standard EN 15804:2012+A2:2019 serves as core
EPD software:
PCR
The Norwegian EPD Foundation LCAno EPD generator ID: 110335
NPCR 030:2021 Part B for ventilation components
1 / 12
General information
Product Owner of the declaration:
TVE-Q TROX Group
Contact person: Alina Buchner
Phone: +49 2845 2020
e-mail: productsustainability-de@troxgroup.com
Program operator: Manufacturer:
The Norwegian EPD Foundation TROX Group
Post Box 5250 Majorstuen, 0303 Oslo, Norway Heinrich-Trox-Platz 1
Phone: +47 977 22 020 47506 Neukirchen-Vluyn, Germany
web: www.epd-norge.no
Declaration number: Place of production:
TROX GmbH - Werk Anholt
Gendringer Str. 85
46419 Isselburg, Germany
This declaration is based on Product Category Rules: Management system:
CEN Standard EN 15804:2012+A2:2019 serves as core PCR ISO 9001, ISO 14001:2015, ISO 50001:2018
NPCR 030:2021 Part B for ventilation components
Statement of liability: Organisation no:
The owner of the declaration shall be liable for the underlying DE 120250070
information and evidence. EPD Norway shall not be liable with respect
to manufacturer information, life cycle assessment data and
evidences.​
Declared unit: Issue date:
1 pcs TVE-Q
Declared unit with option: Valid to:
A1-A3,A4,C1,C2,C3,C4,D
Year of study:
2023
Functional unit: Comparability:
- EPD of construction products may not be comparable if they not
comply with EN 15804 and seen in a building context.
General information on verification of EPD from EPD tools: Development and verification of EPD:
Independent verification of data, other environmental information The declaration is created using EPD tool lca.tools ver EPD2022.03,
and the declaration according to ISO 14025:2010, § 8.1.3 and § 8.1.4. developed by LCA.no. The EPD tool is integrated in the company's
Verification of each EPD is made according to EPD-Norway’s management system and has been approved by EPD Norway.
guidelines for verification and approval requiring that tools are i)
integrated into the company's environmental management system, ii) Developer of EPD: Philipp Ceulaers
the procedures for use of the EPD tool are approved by EPD-Norway,
Reviewer of company-specific input data and EPD:​ Alina Buchner
and iii) the process is reviewed annually by an independent third
party verifier. See Appendix G of EPD-Norway's General Programme
Instructions for further information on EPD tools
Verification of EPD tool: Approved:
Independent third party verification of the EPD tool, background data
and test-EPD in accordance with EPDNorway's procedures and
guidelines for verification and approval of EPD tools.
Third party verifier:
Alexander Borg, Asplan Viak AS
(no signature required)
2 / 12
Product
Product description:
Compact solution for low airflow velocities.
Angular air terminal units for use in variable air terminal systems at low air velocities, even under unfavourable upstream conditions.
For more information see: www.trox.de/en/428f30783cd80fe1
Product specification
VAV terminal units in rectangular design for variable and constant volume flow systems, for supply air or extract air, in several nominal sizes. High
control accuracy of set volume flow rates, even in unfavourable upstream conditions. Control range at least 1:10. Differential pressure
measurement and control via damper blade. Tubeless differential pressure transmission through differential pressure duct in axis Air leakage with
closed damper blade according to EN 1751: Class 3. Casing air leakage according to EN 1751: Class C. Ready-to-commission unit which consists of
the mechanical parts and the factory mounted electronic control component. Position of the damper blade indicated externally at the control
component The damper blade is factory set to open position, which allows a ventilation airflow even without control. Meets the hygiene
requirements of EN 16798, Part 3, of VDI 6022, Sheet 1, and of DIN 1964, Part 4.
This EPD includes the environmental data of the product series TVE-Q.
The following represents a representative dataset of the most sold variant in the declared sales year (TVE-Q/300x200/EASY).
Materials kg %
Electronic - Unspecified 0,62 10,78
Glass fibre reinforced plastic,
0,04 0,68
polyamide
Metal - Aluminium 0,06 1,06
Metal - Galvanized Steel 4,96 86,17
Metal - Stainless steel 0,04 0,73
Plastic - Ethylene vinyl acetate (EVA) 0,00 0,01
Plastic - Polybutylene terephthalate
0,00 0,08
(PBT)
Plastic - Polyurethane (PUR) 0,00 0,01
Product label - supercalendered 0,00 0,01
Rubber, synthetic 0,03 0,47
Total 5,75 100,00
Packaging kg %
Packaging - Cardboard 1,50 27,27
Packaging - Pallet 3,50 63,64
Packaging - Paper 0,50 9,09
Total incl. packaging 11,25 100,00
Technical data:
Nominal sizes: 200 × 100, 300 × 100, 200 × 200, 300 × 200, 400 × 200, 500 × 200, 600 × 200
Volume flow rate range: 16 - 960 l/s or 58 - 3456 m³/h
Volume flow rate control range (controller with dynamic differential pressure measurements): approx. 10 - 100 % of the nominal volume flow rate
Minimum differential pressure: up to 50 Pa (without secondary silencer)
Maximum differential pressure: Control component with dynamic transducer: 900 Pa, Control component with static transducer: 600 Pa
Operating temperature: 10 to 50 °C
For more technical data see: www.trox.de/en/428f30783cd80fe1
The distribution of materials in the products is approximately the same; only the total weight varies. The EPD is created for TVE-Q/300x200. The
factors in the table below can be used to scale LCA data for a new dimension.
Product Weight (kg) Factor
TVE-Q/200x100 3,3 0,63
TVE-Q/300x100 4,1 0,79
TVE-Q/200x200 4,2 0,81
TVE-Q/300x200 5,2 1
TVE-Q/400x200 6,1 1,17
TVE-Q/500x200 7,6 1,46
TVE-Q/600x200 8,3 1,60
Market:
Europe
Reference service life, product
20-25 years.
Reference service life, building or construction works
3 / 12
60 years.
LCA: Calculation rules
Declared unit:
1 pcs TVE-Q
Cut-off criteria:
All major raw materials and all the essential energy is included. The production processes for raw materials and energy flows with very small
amounts (less than 1%) are not included. These cut-off criteria do not​ apply for hazardous materials and substances.
Allocation:
The allocation is made in accordance with the provisions of EN 15804. Energy, water and waste production in-house is allocated equally among all
products through mass allocation. Effects of primary production of recycled materials is allocated to the main product in which the material was
used. The recycling process and transportation of the material is allocated to this analysis.
Data quality:
Specific data for the product composition are provided by the manufacturer. The data represent the production of the declared product and were
collected for EPD development in the year of study. Background data is based on EPDs according to EN 15804 and different LCA databases. The
data quality of the raw materials in A1 is presented in the table below.
Materials Source Data quality Year
Electronic - Unspecified ecoinvent 3.6 Database 2019
Glass fibre reinforced plastic, polyamide Modified ecoinvent 3.6 Database 2019
Metal - Aluminium ecoinvent 3.6 database 2019
Metal - Galvanized Steel ecoinvent 3.6 Database 2020
Metal - Stainless steel ecoinvent 3.6 Database 2019
Packaging - Cardboard ecoinvent 3.6 Database 2019
Packaging - Pallet ecoinvent 3.6 Database 2019
Packaging - Paper ecoinvent 3.6 Database 2019
Plastic - Ethylene vinyl acetate (EVA) ecoinvent 3.6 Database 2019
Plastic - Polybutylene terephthalate (PBT) ecoinvent 3.6 Database 2019
Plastic - Polyurethane (PUR) ecoinvent 3.6 Database 2019
Product label - supercalendered ecoinvent 3.6 Database 2019
Rubber, synthetic ecoinvent 3.6 Database 2019
4 / 12
System boundaries (X=included, MND=module not declared, MNR=module not relevant)
Construction Beyond the system
Product stage Use stage End of life stage
installation stage boundaries
A1 A2 A3 A4 A5 B1 B2 B3 B4 B5 B6 B7 C1 C2 C3 C4 D
X X X X MND MND MND MND MND MND MND MND X X X X X
System boundary:
Additional technical information:
Angular air terminal units for use in variable air terminal systems at low air velocities, even under unfavourable upstream conditions.
Tubeless differential pressure measurement via damper blade.
Differential pressure transmission through differential pressure duct in axis.
Connection terminals with protective cover, no junction box required.
Any airflow direction if dynamic transducer is used.
Suitable for air velocities from 0.8 - 8 m/s.
Compact dimensions for use in confined ceiling areas.
Plug-and-play solution in conjunction with X-AIRCONTROL room control.
Exact measurement even with low airflow velocities.
Any installation orientation also with static transducer.
Closed blade air leakage to EN 1751, at least class 3.
Casing air leakage to EN 1751, class C.
Volume flow rate range 1:10.
Optional equipment and accessories:
Secondary silencer to reduce air-regenerated noise.
Hot water heat exchanger Type WT for reheating the airflow.
waR slairetam tropsnarT gnirutcafunaM tropsnarT ylbmessA e​sU ecnanetniaM riapeR tnemecalpeR tnemhsibrufeR lanoitarepO ygrene esu lanoitarepO esu retaw -eD noitcurtsnoc noitilomed tropsnarT etsaW gnissecorp lasopsiD -yrevoceR-esueR laitnetop-gnilcyceR
5 / 12
LCA: Scenarios and additional technical information
The following information describe the scenarios in the different modules of the EPD.
Capacity utilisation Value
Transport from production place to user (A4) Distance (km) Fuel/Energy Consumption Unit
(incl. return) % (Liter/tonne)
Truck, 16-32 tonnes, EURO 6 (km) 36,7 % 800 0,043 l/tkm 34,40
De-construction demolition (C1) Unit Value
Demolition of building per kg of ventilation
kg/DU 5,75
product (kg)
Capacity utilisation Value
Transport to waste processing (C2) Distance (km) Fuel/Energy Consumption Unit
(incl. return) % (Liter/tonne)
Truck, 16-32 tonnes, EURO 6 (km) 36,7 % 50 0,043 l/tkm 2,15
Waste processing (C3) Unit Value
Materials to recycling (kg) kg 4,56
Waste treatment per kg Electronic scrap,
kg 0,62
incineration (kg)
Waste treatment per kg Hazardous waste,
kg 0,00
incineration (kg)
Waste treatment per kg Plastics, incineration (kg) kg 0,02
Waste treatment per kg Rubber, municipal
kg 0,01
incineration with fly ash extraction (kg)
Disposal (C4) Unit Value
Landfilling of ashes from incineration of
Electronic scrap, process of ashes and residues kg 0,44
(kg)
Landfilling of ashes from incineration of Plastics,
kg 0,00
process per kg ashes and residues (kg)
Landfilling of ashes from incineration of Rubber,
kg 0,00
municipal incineration with fly ash extraction (kg)
Landfilling of ashes from incineration per kg
kg 0,00
Hazardous waste, from incineration (kg)
Waste, aluminium, to landfill (kg) kg 0,00
Waste, plastic, mixture, to landfill (kg) kg 0,04
Waste, scrap steel, to landfill (kg) kg 0,50
Benefits and loads beyond the system
Unit Value
boundaries (D)
Substitution of electricity (MJ) MJ 0,02
Substitution of primary aluminium with net scrap
kg 0,05
(kg)
Substitution of primary steel with net scrap (kg) kg 1,04
Substitution of thermal energy, district heating
MJ 0,28
(MJ)
6 / 12
LCA: Results
The LCA results are presented below for the declared unit defined on page 2 of the EPD document.
Environmental impact
Indicator Unit A1-A3 A4 C1 C2 C3 C4 D
GWP-total kg CO2 -eq 4,23E+01 1,47E+00 7,58E-03 9,20E-02 7,50E-01 5,82E-02 -1,65E+00
GWP-fossil kg CO2 -eq 5,04E+01 1,47E+00 7,58E-03 9,19E-02 7,49E-01 5,81E-02 -1,64E+00
GWP-biogenic kg CO2 -eq -8,15E+00 6,08E-04 1,42E-06 3,80E-05 9,73E-05 8,16E-05 -2,87E-03
GWP-luluc kg CO2 -eq 9,12E-02 5,23E-04 5,98E-07 3,27E-05 2,27E-05 2,05E-05 -9,78E-03
ODP kg CFC11 -eq 4,43E-06 3,33E-07 1,64E-09 2,08E-08 3,80E-09 3,48E-09 -1,18E-04
AP mol H+ -eq 4,42E-01 4,22E-03 7,93E-05 2,64E-04 2,56E-04 1,19E-04 -9,01E-03
EP-FreshWater kg P -eq 6,19E-03 1,17E-05 2,76E-08 7,34E-07 8,26E-07 6,58E-07 -8,96E-05
EP-Marine kg N -eq 6,25E-02 8,36E-04 3,50E-05 5,22E-05 1,07E-04 3,65E-05 -1,60E-03
EP-Terrestial mol N -eq 1,16E+00 9,35E-03 3,84E-04 5,84E-04 1,09E-03 3,58E-04 -1,67E-02
POCP kg NMVOC -eq 2,08E-01 3,58E-03 1,06E-04 2,24E-04 2,69E-04 1,00E-04 -7,31E-03
ADP-minerals&metals1 kg Sb-eq 3,09E-02 4,06E-05 1,16E-08 2,54E-06 2,92E-07 2,53E-07 -1,91E-05
ADP-fossil1 MJ 6,76E+02 2,22E+01 1,04E-01 1,39E+00 3,24E-01 3,13E-01 -1,59E+01
WDP1 m3 3,08E+03 2,15E+01 2,22E-02 1,34E+00 9,43E-01 9,48E-01 -2,19E+02
GWP-total = Global Warming Potential total; GWP-fossil = Global Warming Potential fossil fuels; GWP-biogenic = Global Warming Potential biogenic; GWP-luluc =
Global Warming Potential land use and land use change; ODP = Depletion potential of the stratospheric ozone layer; AP = Acidification potential, Accumulated
Exceedance; EP-freshwater = Eutrophication potential, fraction of nutrients reaching freshwater end compartment: EP-marine = Eutrophication potential, fraction of
nutrients reaching marine end compartment; EP-terrestrial = Eutrophication potential, Accumulated Exceedance; POCP = Formation potential of tropospheric ozone;
ADP-minerals&metals = Abiotic depletion potential for non-fossil resources; ADP-fossil = Abiotic depletion for fossil resources potential; WDP = Water (user)
deprivation potential, deprivation-weighted water consumption
"Reading example: 9,0 E-03 = 9,0*10-3 = 0,009"
*INA Indicator Not Assessed
1. The results of this environmental impact indicator shall be used with care as the uncertainties on these results are high or as there is limited experienced with the
indicator
Remarks to environmental impacts
7 / 12
Additional environmental impact indicators
Indicator Unit A1-A3 A4 C1 C2 C3 C4 D
PM Disease incidence 3,86E-06 9,00E-08 2,10E-09 5,63E-09 1,57E-09 1,47E-09 -1,30E-07
IRP2 kgBq U235 -eq 2,79E+00 9,72E-02 4,47E-04 6,07E-03 1,19E-03 1,37E-03 -2,28E-02
ETP-fw1 CTUe 3,30E+03 1,65E+01 5,70E-02 1,03E+00 2,16E+00 4,19E+00 -7,15E+01
HTP-c1 CTUh 1,60E-07 0,00E+00 0,00E+00 0,00E+00 6,10E-11 1,10E-11 -6,76E-09
HTP-nc1 CTUh 2,84E-06 1,80E-08 5,20E-11 1,13E-09 5,51E-09 5,47E-10 1,06E-07
SQP1 dimensionless 9,82E+02 1,55E+01 1,32E-02 9,72E-01 1,18E-01 4,04E-01 -9,31E-01
PM = Particulate Matter emissions; IRP = Ionizing radiation – human health; ETP-fw = Eco toxicity – freshwater; HTP-c = Human toxicity – cancer effects; HTP-nc =
Human toxicity – non cancer effects; SQP = Potential Soil Quality Index (dimensionless)
"Reading example: 9,0 E-03 = 9,0*10-3 = 0,009"
*INA Indicator Not Assessed
1. The results of this environmental impact indicator shall be used with care as the uncertainties on these results are high or as there is limited experienced with the
indicator
2. This impact category deals mainly with the eventual impact of low dose ionizing radiation on human health of the nuclear fuel cycle. It does not consider effects due
to possible nuclear accidents, occupational exposure nor due to radioactive waste disposal in underground facilities. Potential ionizing radiation from the soil, from
radon and from some construction materials is also not measured by this indicator.
8 / 12
Resource use
Indicator Unit A1-A3 A4 C1 C2 C3 C4 D
PERE MJ 1,19E+02 3,18E-01 5,64E-04 1,99E-02 2,24E-02 1,95E-02 -3,16E+00
PERM MJ 6,79E+01 0,00E+00 0,00E+00 0,00E+00 0,00E+00 0,00E+00 0,00E+00
PERT MJ 1,87E+02 3,18E-01 5,64E-04 1,99E-02 2,24E-02 1,95E-02 -3,16E+00
PENRE MJ 6,74E+02 2,22E+01 1,04E-01 1,39E+00 3,24E-01 3,14E-01 -1,59E+01
PENRM MJ 2,09E+00 0,00E+00 0,00E+00 0,00E+00 0,00E+00 0,00E+00 0,00E+00
PENRT MJ 6,76E+02 2,22E+01 1,04E-01 1,39E+00 3,24E-01 3,14E-01 -1,59E+01
SM kg 4,52E+00 0,00E+00 5,12E-05 0,00E+00 0,00E+00 3,94E-06 0,00E+00
RSF MJ 2,86E+00 1,14E-02 1,39E-05 7,11E-04 5,45E-04 4,64E-04 4,06E-02
NRSF MJ 9,81E+00 4,07E-02 2,04E-04 2,54E-03 -3,88E-04 1,35E-04 1,20E+00
FW m3 5,79E-01 2,38E-03 5,37E-06 1,49E-04 1,49E-03 1,22E-03 -1,48E-02
PERE = Use of renewable primary energy excluding renewable primary energy resources used as raw materials; PERM = Use of renewable primary energy resources used
as raw materials; PERT = Total use of renewable primary energy resources; PENRE = Use of non renewable primary energy excluding non-renewable primary energy
resources used as raw materials; PENRM = Use of non renewable primary energy resources used as raw materials; PENRT = Total use of non renewable primary energy
resources; SM = Use of secondary materials; RSF = Use of renewable secondary fuels; NRSF = Use of non-renewable secondary fuels; FW = Net use of fresh water
"Reading example: 9,0 E-03 = 9,0*10-3 = 0,009"
*INA Indicator Not Assessed
9 / 12
End of life - Waste
Indicator Unit A1-A3 A4 C1 C2 C3 C4 D
HWD kg 3,61E-01 1,15E-03 3,07E-06 7,16E-05 2,06E-03 1,37E-02 -3,93E-03
NHWD kg 1,24E+01 1,08E+00 1,24E-04 6,76E-02 2,94E-01 8,40E-01 -6,11E-01
RWD kg 2,38E-03 1,51E-04 7,25E-07 9,46E-06 1,18E-06 1,12E-06 -2,22E-05
HWD = Hazardous waste disposed; NHWD = Non-hazardous waste disposed; RWD = Radioactive waste disposed
"Reading example: 9,0 E-03 = 9,0*10-3 = 0,009"
*INA Indicator Not Assessed
End of life - Output flow
Indicator Unit A1-A3 A4 C1 C2 C3 C4 D
CRU kg 0,00E+00 0,00E+00 0,00E+00 0,00E+00 0,00E+00 0,00E+00 0,00E+00
MFR kg 7,51E-01 0,00E+00 5,03E-05 0,00E+00 4,56E+00 3,21E-06 0,00E+00
MER kg 1,01E-04 0,00E+00 1,56E-07 0,00E+00 1,43E-02 7,86E-08 0,00E+00
EEE MJ 2,20E-02 0,00E+00 5,35E-07 0,00E+00 3,67E-01 5,10E-06 0,00E+00
EET MJ 3,32E-01 0,00E+00 8,09E-06 0,00E+00 5,56E+00 7,72E-05 0,00E+00
CRU = Components for re-use; MFR = Materials for recycling; MER = Materials for energy recovery; EEE = Exported energy electrical; EET = Exported energy thermal
"Reading example: 9,0 E-03 = 9,0*10-3 = 0,009"
*INA Indicator Not Assessed
Biogenic Carbon Content
Indicator Unit At the factory gate
Biogenic carbon content in product kg C 2,25E-04
Biogenic carbon content in accompanying packaging kg C 2,38E+00
Note: 1 kg biogenic carbon is equivalent to 44/12 kg CO2
10 / 12
Additional requirements
Greenhouse gas emissions from the use of electricity in the manufacturing phase
National production mix from import, low voltage (production of transmission lines, in addition to direct emissions and losses in grid) of applied
electricity for the manufacturing process (A3).
Electricity mix Source Amount Unit
Electricity, market mix (kWh) - Germany ecoinvent 3.6 585,93 g CO2-eq/kWh
Dangerous substances
The product contains dangerous substances, more than 0,1% by weight, given by the REACH Candidate List, see table:
Name CASNo Amount
Lead 7439-92-1 > 0.1% w/w
Indoor environment
Additional Environmental Information
Additional environmental impact indicators required in NPCR Part A for construction products
Indicator Unit A1-A3 A4 C1 C2 C3 C4 D
GWPIOBC kg CO2 -eq 5,10E+01 1,47E+00 7,58E-03 9,19E-02 7,50E-01 5,19E-02 -2,20E+00
GWP-IOBC: Global warming potential calculated according to the principle of instantaneous oxidation. In order to increase the transparency of biogenic carbon​
contribution to climate impact, the indicator GWP-IOBC is required as it declares climate impacts calculated according to the principle of instantaneous oxidation.​
GWP-IOBC is also referred to as GWP-GHG in context to Swedish public procurement legislation.
11 / 12
Bibliography
ISO 14025:2010 Environmental labels and declarations - Type III environmental declarations - Principles and procedures.
ISO 14044:2006 Environmental management - Life cycle assessment - Requirements and guidelines.
EN 15804:2012+A2:2019 Environmental product declaration - Core rules for the product category of construction products.
ISO 21930:2017 Sustainability in buildings and civil engineering works - Core rules for environmental product declarations of construction
products.
ecoinvent v3, Allocation, cut-off by classification, Swiss Centre of Life Cycle Inventories.
Iversen et al., (2021) eEPD v2021.09 Background information for EPD generator tool system verification, LCA.no Report number: 07.21
Graafland and Iversen (2022) EPD generator for NPCR 030 Ventilation components, Background information for EPD generator application and
LCA data, LCA.no report number: 12.22
NPCR Part A: Construction products and services. Ver. 2.0. April 2021, EPD-Norge.
NPCR 030 Part B for Ventilation components, Ver. 1.0, 18.05.2021, EPD Norway.
EN ISO 9001:2015 - Quality management systems
EN ISO 14001:2015 - Environmental management systems
EN ISO 50001:2018 - Energy management systems
Program operator and publisher Phone: +47 977 22 020
The Norwegian EPD Foundation e-mail: post@epd-norge.no
Post Box 5250 Majorstuen, 0303 Oslo, Norway web: www.epd-norge.no
Owner of the declaration: Phone: +49 2845 2020
productsustainability-
TROX Group e-mail:
de@troxgroup.com
Heinrich-Trox-Platz 1, 47506 Neukirchen-Vluyn web: https://www.trox.de/en
Author of the Life Cycle Assessment Phone: +47 916 50 916
LCA.no AS e-mail: post@lca.no
Dokka 6A, 1671 web: www.lca.no
Developer of EPD generator Phone: +47 916 50 916
LCA.no AS e-mail: post@lca.no
Dokka 6B,1671 Kråkerøy web: www.lca.no
ECO Platform web: www.eco-platform.org
ECO Portal web: ECO Portal
12 / 12
