ENVIRONMENTAL PRODUCT DECLARATION
as per ISO 14025 and EN 15804+A1
Owner of the Declaration dormakaba International Holding GmbH
Publisher Institut Bauen und Umwelt e.V. (IBU)
Programme holder Institut Bauen und Umwelt e.V. (IBU)
Declaration number EPD-DOR-20200384-CBD3-EN
Issue date 24/08/2020
Valid to 23/08/2025
8600 and 8900 Series door closers
dormakaba
www.ibu-epd.com | https://epd-online.com
General Information
dormakaba 8600 and 8900 Series door closers
Programme holder Owner of the declaration
IBU – Institut Bauen und Umwelt e.V. dormakaba International Holding GmbH
Hegelplatz 1 DORMA Platz 1
10117 Berlin 58256 Ennepetal
Germany Germany
Declaration number Declared product / declared unit
EPD-DOR-20200384-CBD3-EN The declaration represents one surface applied door closer unit (8600 and
8900 Series).
This declaration is based on the product category rules: Scope:
Building Hardware products, 01/08/2021 The declaration and the background LCA represent dormakaba's 8600 and
(PCR checked and approved by the SVR) 8900 Series door closers. Raw materials are provided by suppliers, but the
closers are manufactured and assembled at dormakaba facilities
worldwide. Closer bodies are manufactured at dormakaba's Singapore
Issue date facility and components of the closer arm are manufactured at dormakaba
facilities in Ennepetal, Germany and Steelville, USA. These parts are then
24/08/2020
shipped to Reamstown, USA, where the final assembly takes place.
The owner of the declaration shall be liable for the underlying information
and evidence; the IBU shall not be liable with respect to manufacturer
Valid to
information, life cycle assessment data and evidences.
23/08/2025
The EPD was created according to the specifications of EN 15804+A1. In
the following, the standard will be simplified as EN 15804.
Verification
The standard EN 15804 serves as the core PCR
Independent verification of the declaration and data according to ISO
14025:2011
internally X externally
Dipl.-Ing. Hans Peters
(Chairman of Institut Bauen und Umwelt e.V.)
Florian Pronold Dr.-Ing. Wolfram Trinius,
(Managing Director Institut Bauen und Umwelt e.V.) (Independent verifier)
1 Environmental Product Declaration - dormakaba - 8600 and 8900 Series door closers
Product
like ANSI A156.4 Grade 1, UL 10C, and ANSI A117.1. The
Product description/Product definition closers are also Underwriters Laboratories (label for the US,
The 8600 and 8900 Series door closers are non-handed UL) and Label for Canada (CUL) listed, and CSFM (California
surface applied door closers with adjustable spring power (size State Fire Marshall) approved. The plants in Singapore and
1-6) and backcheck that controls opening motion during Ennepetal are certified to the quality management system ISO
abusive or abrupt opening. 9001, which ensures consistent quality of dormakaba's
Supported by a full complement of optional arms, plates, and products.
brackets, the door closers provide the flexibility needed to meet
the demands of commercial and institutional applications, The Environmental Management System in the Singapore
including Americans with Disabilities Act (ADA) barrier-free production is certified to ISO 14001 and the Energy
accessibility requirements. The door closers are available with Management to ISO 50001. The dormakaba Environmental
slim plastic, full plastic and full metal cover. For the use and Management system at the Ennepetal facility is certified to ISO
application of the product the respective national provisions at 14001. Occupational Health and Safety is certified to OHSAS
the place of use apply. The standards which can be applied are 18001 and Energy Management to ISO 50001.
the following:
Base materials/Ancillary materials
• ANSI/BHMA 156.4
• ANSI/ICC A117.1 Name Value Unit
• UL listed product Steel 62 %
• UL 10C Aluminum 24 %
• ADA compliant (version 1-6)
Oil 6 %
Application Plastics 5 %
The 8600 and 8900 Series door closers are designed for Coatings 2 %
commercial and institutional applications, including ADA barrier- Other 1 %
free accessibility requirements.
The products include partial articles which contain substances
They are suitable for use on hollow metal, aluminum and wood
listed in the Candidate List of REACH Regulation
doors and can be used for fire doors.
1907/2006/EC (date: 15.01.2019) exceeding 0.1 percentage by
Technical Data mass in the alloy:
The 8600 and 8900 Series have two independent adjustment
• Lead (Pb): 7439-290-1 (CAS-No.)
valves to control the closing speed from 180° - 10° and from
The Candidate List can be found on the ECHA website
10° - 0°. Optional delayed action adjustable with a separate
address: https://echa.europa.eu/de/home.
independent valve delays door closing to allow unobstructed
passage through the opening.
Reference service life
Based on arm selection, the mounting options are regular (pull
The reference service life of dormakaba's 8600 and 8900
side of the door), top jamb (push side of the door) and parallel
Series door closers depends on the traffic pattern and degree
arm (push side of the door).
of usage of the door. These closers are rated to ANSI Grade 1,
meaning they are designed to withstand a minimum of
Performance data of the product with respect to its
1,500,000 cycles. The reference
characteristics in accordance with the relevant technical
service life amounts for 20 years.
provision which can be applied include product certifications
LCA: Calculation rules
Type of EPD: cradle to gate - with options.
Declared Unit
The declared unit of this analysis is one surface applied door The Environmental Product Declaration refers to the production
closer. stage (A1-A3), transport from the gate to construction site (A4),
Declared unit the end of life stage (C3) and indicates the recycling potential
which is declared in the module "benefits and loads beyond the
Name Value Unit
product system boundary" (D).
Declared unit (1 closer) 1 piece/product
Mass of system (without packaging) 3.0 kg In line with the PCR, A5 is declared to ensure the export of
Conversion factor to 1 kg 0.333 - biogenic CO2 from renewable packaging materials.
Mass of declared Product 3 kg
Modules A1 to A3 include the provision and processing of raw
For IBU core EPDs (where clause 3.6 is part of the EPD): for
materials as well as the
average EPDs, an estimate of the robustness of the LCA
processing of input materials, the transport to manufacturer and
values must be made, e.g. concerning the variability of the
production site. Module C3 includes the incineration of plastics
production process, geographical representativeness and the
for energy recovery. Module D comprises the recycling of
influence of background data and preliminary products
metals and gives the recycling potentials as well as potential
compared to the environmental impacts caused by the actual
benefits from energy substitution.
production.
A5 is declared to ensure the export of biogenic CO2 that is
incorporated in the used packaging materials (paper). Potential
System boundary
benefits from the incineration of packaging materials are also
declared in module D. The incineration processes in the End-of-
2 Environmental Product Declaration - dormakaba - 8600 and 8900 Series door closers
Life are based on European datasets. The recycling processes
in the End-of-Life are based on mainly European datasets. Comparability
Basically, a comparison or an evaluation of EPD data is only
Geographic Representativeness possible if all the data sets to be compared were created
Land or region, in which the declared product system is according to EN 15804 and the building context, respectively
manufactured, used or handled at the end of the product´s the product-specific characteristics of performance, are taken
lifespan: Germany into account.
LCA: Scenarios and additional technical information
Additional technical information for the declared modules. In case a reference service life according to applicable ISO
standards is declared then the assumptions and in-use
Transport to the building site (A4)
conditions underlying the determined RSL shall be declared. In
Name Value Unit
addition, it shall be stated that the RSL applies to the reference
Litres of fuel truck (per piece) 0.006 l/100km conditions only.
Transport distance average (ship) 13000 km
Transport distance average (truck) 1900 km The same holds for a service life declared by the manufacturer.
Corresponding information related to in-use conditions needs
Transport distance range (truck) 10 - 4600 km
not be provided if a service life taken from the list of service life
Transport distance range (ship) 0 - 21900 km
by BNB is declared.
Capacity utilisation (including empty runs) 85 %
In order to represent dormakaba's global distribution network, a End of life (C1-C4)
sales-weighted average is used to model transport to the
Name Value Unit
building site. The table for Module A4 shows both weighted
Recycling 3 kg
average transportation distance (given regional surface closer
sales), which is used in the analysis.
Reuse, recovery and/or recycling potentials (D), relevant
scenario information
Installation into the building (A5) Name Value Unit
Name ValueUnit Recycling 100 %
Output substances following waste treatment on
0.257 kg Collection rate is 100%.
site (packaging)
3 Environmental Product Declaration - dormakaba - 8600 and 8900 Series door closers
LCA: Results
The table below summarizes which modules are declared (as indicated by an "X"), and which are not declared (as indicated with
"MND").
DESCRIPTION OF THE SYSTEM BOUNDARY (X = INCLUDED IN LCA; MND = MODULE NOT DECLARED; MNR = MODULE NOT
RELEVANT)
Benefits and
Construction loads beyond
Product stage Use stage End of life stage
process stage the system
boundaries
la ire ta m w a Ry lp p u s tro p s n a rT g n iru tc a fu n a M e h t m o rf tro p s n a rTe tis e h t o t e ta g y lb m e s s A e s U e c n a n e tn ia M ria p e R tn e m e c a lp e R tn e m h s ib ru fe R y g re n e la n o ita re p Oe s u re ta w la n o ita re p Oe s u n o itc u rts n o c -e Dn o itilo m e d tro p s n a rT g n is s e c o rp e ts a W la s o p s iD -e s u e R-y re v o c e R-g n ilc y c e Rla itn e to p
A1 A2 A3 A4 A5 B1 B2 B3 B4 B5 B6 B7 C1 C2 C3 C4 D
X X X X X MND MND MNR MNR MNR MND MND MND MND X MND X
RESULTS OF THE LCA - ENVIRONMENTAL IMPACT according to EN 15804+A1: 1 closer (3.0kg)
Parameter Unit A1-A3 A4 A5 C3 D
Global warming potential (GWP) kg CO 2 eq 2.47E+01 8.31E-01 1.06E-01 6.24E-01 -1E+01
Depletion potential of the stratospheric ozone layer (ODP) kg CFC11 eq 1.13E-12 6.74E-17 2.56E-17 3.58E-16 1.03E-13
Acidification potential of land and water (AP) kg SO 2 eq 1.03E-01 1.79E-02 2.22E-05 1.48E-04 -3.82E-02
Eutrophication potential (EP) kg PO 43 eq 7.62E-03 2.05E-03 4.19E-06 1.7E-05 -2.53E-03
Formation potential of tropospheric ozone photochemical oxidants (POCP) kg Ethen eq 9.56E-03 4.48E-04 1.47E-06 7.07E-06 -2.82E-03
Abiotic depletion potential for non fossil resources (ADPE) kg Sb eq 8.58E-05 2.76E-08 2.09E-09 6.01E-08 -2.5E-05
Abiotic depletion potential for fossil resources (ADPF) MJ 2.72E+02 1.09E+01 2.95E-02 2.73E-01 -9.67E+01
RESULTS OF THE LCA - INDICATORS TO DESCRIBE RESOURCE USE according to EN 15804+A1: 1 closer (3.0kg)
Parameter Unit A1-A3 A4 A5 C3 D
Renewable primary energy as energy carrier (PERE) MJ 9.45E+00 4.14E-02 4.46E+00 6.55E-02 -2.94E+01
Renewable primary energy resources as material utilization (PERM) MJ 4.46E+00 0 -4.46E+00 0 0
Total use of renewable primary energy resources (PERT) MJ 1.39E+01 4.14E-02 5.9E-03 6.55E-02 -2.94E+01
Non renewable primary energy as energy carrier (PENRE) MJ 2.74E+02 1.09E+01 3.45E-02 2.08E-01 -1.07E+02
Non renewable primary energy as material utilization (PENRM) MJ 9.9E-02 0 0 9.9E-02 0
Total use of non renewable primary energy resources (PENRT) MJ 2.74E+02 1.09E+01 3.45E-02 3.07E-01 -1.07E+02
Use of secondary material (SM) kg 2.54E-01 0 0 0 0
Use of renewable secondary fuels (RSF) MJ 0 0 0 0 0
Use of non renewable secondary fuels (NRSF) MJ 0 0 0 0 0
Use of net fresh water (FW) m3 9.54E-02 1.89E-04 3.1E-04 1.88E-03 -9E-02
RESULTS OF THE LCA – WASTE CATEGORIES AND OUTPUT FLOWS according to EN 15804+A1:
1 closer (3.0kg)
Parameter Unit A1-A3 A4 A5 C3 D
Hazardous waste disposed (HWD) kg 8.88E-06 1.42E-09 6.66E-11 1.99E-09 -1.16E-07
Non hazardous waste disposed (NHWD) kg 3.1E+00 8.42E-05 3.33E-03 6.43E-02 -1.64E+00
Radioactive waste disposed (RWD) kg 8.32E-04 3.87E-06 2E-06 1.35E-05 -4.15E-03
Components for re-use (CRU) kg 0 0 0 0 0
Materials for recycling (MFR) kg 0 0 0 2.95E+00 0
Materials for energy recovery (MER) kg 0 0 0 0 0
Exported electrical energy (EEE) MJ 0 0 1.61E-01 1.2E+00 0
Exported thermal energy (EET) MJ 0 0 2.92E-01 2.31E+00 0
References
ADA CSFM
Americans with Disabilities Act 1990 California State Fire Marshall
ANSI/ICC A117.1 ECHA
ANSI/ICC A117.1 - 2009, Accessible and usable buildings and European Chemicals Agency
facilities
EN 15804
ANSI/BHMA A156.4 EN 15804:2012-04
ANSI/BHMA A156.4 - 2013, Door controls - Closers
Sustainability of construction works - Environmental product
Candidate List of REACH Regulation /1907/2006/EC (date: declarations - Core rules for the product category of
16.01.2020) construction
products
4 Environmental Product Declaration - dormakaba - 8600 and 8900 Series door closers
Institut Bauen und Umwelt e.V., Product Category Rules for
GaBi ts Construction Products from the range of Environmental Product
thinkstep AG, GaBi Software System and Database for Life Declarations of Institut Bauen und Umwelt (IBU), Part A:
Cycle Engineering (SP39). 1992-2019. Copyright thinkstep AG Calculation Rules for the Life Cycle Assessment and
Requirements on the Background Report
ISO 9001
Quality Management System - ISO 9001:2015 PCR Part B
PCR Guidance-Texts for Building-Related Products and
ISO 14001 Services. From the range of
Environmental Management System - ISO 14001:2015 Environmental Product Declarations of Institute Construction
and Environment
ISO 14040 e.V. (IBU). Part B: Requirements on the EPD for building
EN ISO 14040:2006, Environmental management - Life cycle hardware products
assessment - Principles and framework
REACH
ISO 14044 Registration, Evaluation, Authorisation and Restriction of
EN ISO 14044:2006 Environmental management - Life cycle Chemicals (REACH), Regulation (EC) No
assessment - Requirements and guidelines 1907/2006
ISO 50001 UL 10C
Energy Management System - ISO 50001:2011 UL 10C, Positive pressure fire tests of door assemblies
The literature referred to in the Environmental Product
OHSAS 18001 Declaration must be listed in full.Standards already fully quoted
Occupational Health and Safety - OHSAS 18001:2007 in the EPD do not need to be listed here again.
The current version of PCR Part A and PCR Part B of the PCR
PCR Part A document on which they are based must be referenced.
5 Environmental Product Declaration - dormakaba - 8600 and 8900 Series door closers
Publisher
Institut Bauen und Umwelt e.V. +49 (0)30 3087748- 0
Hegelplatz 1 info@ibu-epd.com
10117 Berlin www.ibu-epd.com
Germany
Programme holder
Institut Bauen und Umwelt e.V. +49 (0)30 3087748- 0
Hegelplatz 1 info@ibu-epd.com
10117 Berlin www.ibu-epd.com
Germany
Author of the Life Cycle Assessment
Sphera Solutions GmbH +49 (0)711 341817-0
Hauptstraße 111- 113 info@sphera.com
70771 Leinfelden-Echterdingen www.sphera.com
Germany
Owner of the Declaration
dormakaba International Holding GmbH +49 2333 793-0
DORMA Platz 1 info.de@dormakaba.com
58256 Ennepetal www.dormakaba.com
Germany
6 Environmental Product Declaration - dormakaba - 8600 and 8900 Series door closers
