ENVIRONMENTAL PRODUCT DECLARATION
as per ISO 14025 and EN 15804+A2
Owner of the Declaration ARGE – The European Federation of Locks and Building Hardware Manufacturers
Publisher Institut Bauen und Umwelt e.V. (IBU)
Programme holder Institut Bauen und Umwelt e.V. (IBU)
Declaration number EPD-ARG-20230542-IBG1-EN
Issue date 02.04.2024
Valid to 01.04.2029
Door and window handles
ARGE – The European Federation of Locks
and Building Hardware Manufacturers
This EPD is valid only for products supplied by an ARGE EPD licence holder.
www.ibu-epd.com | https://epd-online.com
1. General Information
ARGE – The European Federation of Locks Door and window handles
and Building Hardware Manufacturers
Programme holder Owner of the declaration
IBU – Institut Bauen und Umwelt e.V. ARGE – The European Federation of Locks and Building Hardware
Hegelplatz 1 Manufacturers
10117 Berlin Offerstraße 12
Germany 42551 Velbert
Germany
Declaration number Declared product / declared unit
EPD-ARG-20230542-IBG1-EN 1 kg of door or window handle
This declaration is based on the product category rules: Scope:
Building Hardware products, 01.08.2021 This ARGE EPD covers handles intended to be used in door and window
(PCR checked and approved by the SVR) assemblies of varying materials and applications. The reference product
used to calculate the impact this product group has on the environment is
a door handle composed primarily of brass and steel and has been
Issue date selected for the LCA (Life Cycle Assessment) because it is the product with
the highest impact for 1 kg of product. A validity scope analysis has also
02.04.2024
been carried out to determine the limiting factors for door and window
handles covered by this EPD. In a preliminary study (simplified LCA), it has
been confirmed that this EPD represents the worst-case condition and it
Valid to
can therefore be used to cover all door and window handles manufactured
01.04.2029 in Europe by ARGE member companies.
The owner of the declaration shall be liable for the underlying information
and evidence; the IBU shall not be liable with respect to manufacturer
information, life cycle assessment data and evidences.
The EPD was created according to the specifications of EN 15804+A2. In
the following, the standard will be simplified as EN 15804.
Verification
The standard EN 15804 serves as the core PCR
Independent verification of the declaration and data according to ISO
14025:2011
Dipl.-Ing. Hans Peters
(Chairman of Institut Bauen und Umwelt e.V.) internally X externally
Florian Pronold Dr. Matthew Fishwick,
(Managing Director Institut Bauen und Umwelt e.V.) (Independent verifier)
1 Environmental Product Declaration - ARGE – The European Federation of Locks and Building Hardware Manufacturers - Door and window handles
2. Product
Steel is produced by combining iron with carbon as well as
2.1 Product description/Product definition
other elements depending on the desired characteristics.
This EPD covers handle mechanisms for the opening and Components made of steel are formed by different types of
maintaining in a closed position of doors or windows in mechanical processing.
buildings.
For the application and use the respective national provisions PEHD (polyethylene high-density) is a thermoplastic polymer
at the place of use apply. produced from the monomer ethylene. Components made of
PEHD are formed by injection moulding or other thermal
2.2 Application
forming processes.
These products are designed to be integrated into door or
window assemblies consisting of various materials and used for Acetal, or polyoxymethylene (POM), is produced by
various applications. They may be used on all kinds of doors polymerisation of anhydrous formaldehyde. Components made
and windows (both inside and outside). of Acetal are formed by injection moulding or other thermal
forming processes.
2.3 Technical Data
Ideally, products should comply with a suitable technical
Aluminium is a non-ferrous metal produced from bauxite by
specification. EN 1906 and EN 13126 are examples of such
the Bayer process. Components made of aluminium are
specifications and some products will comply with them. The
manufactured by extrusion or other types of mechanical
relevant grading structure according to EN 1906 is shown in the
processing.
following table:
Name Value Unit
Stainless steel is produced by combining iron with chromium
Category of use 1 - 4 Grade as well as other elements depending on the desired
Durability 6, 7 Grade characteristics. Components made of steel are formed by
Test door mass - Grade stamping or other types of mechanical processing.
Suitability for fire resistance & 0, A, A1, B, B1, C,
Grade Nylon 6 is a polymer, in particular polyamide. It is formed by
smoke control doors C1, D, D1
the ring-opening polymerisation of caprolactam. Components
Safety 0, 1 Grade
made of Nylon 6 are formed by injection moulding or other
Corrosion resistance 0 – 5 Grade thermal forming processes.
Security – burglar resistance 0 – 4 Grade
Type of operation A, B, U Grade Nylon 66 is a polymer, in particular polyamide. It is formed by
the polycondensation of hexamethylenediamine and adipic acid
Performance data of the product with respect to its
in equal parts. Components made of Nylon 66 are formed by
characteristics in accordance with the relevant technical
injection moulding or other thermal forming processes.
provision (no CE-marking).
Zamak is an alloy with a base metal of zinc and alloying
2.4 Delivery status
elements of aluminium, magnesium, and copper. Components
The products are sold by unit. Deliveries of individual items are
made of Zamak are die-cast.
possible but are an exception. Standard deliveries comprise a
larger quantity of handles, as they are marketed as "B2B"
Zinc is a slightly brittle metal. Zinc is used as an anti-corrosion
products and not to end-users.
agent when galvanising components made of steel.
2.5 Base materials/Ancillary materials
Epoxy is the family of basic components or cured end products
Composition of product analysed for this EPD:
of epoxy resins, also known as polyepoxides. Epoxy may be
used e.g., as an adhesive, sealant or for coating components.
The values given in the table below are for the product
analysed for this EPD. Ranges of values for other products
1) This product/article/at least one partial article contains
covered by the validity scope analysis are shown in brackets.
substances listed in the ECHA candidate list (date: 14.06.2023)
Name Value Unit
exceeding 0.1 percentage by mass: Certain components may
Brass (0.00% – 74.15%) 74.15 % contain small amounts of lead (CAS no. 7439-92-1) as an
Steel (0.00% – 89.48%) 24.97 % alloying element.
PEHD (polyethylene high density) (0.00% – 0.65%) 0.61 %
2) This product/article/at least one partial article contains other
Acetal (POM - polyoxymethylene) (0.00% – 8.51%) 0.27 %
cancerogenic, mutagenic, reprotoxic (CMR) substances in
Aluminium (0.00% – 68.97%) 0 %
categories 1A or 1B which are not on the ECHA candidate list,
Stainless steel (0.00% – 62.45%) 0 % exceeding 0.1 percentage by mass: no.
Nylon 6 (0.00% – 27.54%) 0 %
Nylon 66 (0.00% – 0.21%) 0 % 3) Biocide products were added to this construction product or it
has been treated with biocide products (this then concerns a
Zamak (0.00% – 9.24%) 0 %
treated product as defined by the (EU) Ordinance on Biocide
Zinc (0.00% – 93.41%) 0 %
Products No. 528/2012): no.
Epoxy (0.00% – 18.19%) 0 %
2.6 Manufacture
Brass is an alloy of zinc and copper. Components made of
The production of a handle normally follows a 3-step
brass are made by forging, die-casting or other types of
procedure:
mechanical processing.
2 Environmental Product Declaration - ARGE – The European Federation of Locks and Building Hardware Manufacturers - Door and window handles
The reference service life is 30 years under normal working
1. Manufacture of components: this step might include a
conditions. This corresponds to passing a mechanical
surface treatment in the factory or by external
endurance test of 100.000 cycles as specified in the EN 1906.
contractors.
The reference service life is dependent on the actual frequency
2. Preassembly of modules (in the factory).
of use and environmental conditions. It is required that
3. Final assembly (in the factory).
installation, as well as maintenance of the product, must be
2.7 Environment and health during manufacturing done in line with instructions provided by the manufacturer.
Regular measurements of air quality and noise levels are
2.13 Extraordinary effects
carried out by the manufacturers, the ARGE member
Fire
companies. The results shall be within the mandatory safety
In general, the product is suitable for use in a fire resisting
levels. In areas where employees are exposed to chemical
and/or smoke control door/window sets according to the
products, the required protective clothing and technical
classes specified in EN 1906, unless it is classified in
protective devices shall be provided. Regular health checks are
class/grade 0.
mandatory for employees in production facilities.
2.8 Product processing/Installation Water
The installation of the product may vary depending on the type The declared product is intended to be used in buildings under
of door or window and the specific situation, but the products normal conditions (indoor or outdoor use). It shall not emit
shall not require energy consumption for installation. hazardous substances in the event of flooding.
2.9 Packaging Mechanical destruction
Normally, each individual product is packed in paper or Mechanical destruction of the declared product shall not
cardboard. These individual products are then packed in a materially alter its composition, or have any adverse effect on
cardboard box and stacked on wooden pallets for transport to the environment.
the customer.
2.14 Re-use phase
Waste from product packaging is collected separately for waste Removal of door or window handle components (for re-use or
disposal (including recycling). recycling) shall have no adverse effect on the environment.
2.10 Condition of use 2.15 Disposal
Once installed, the products shall require no servicing during Door or window handle components should be recycled
their expected service lives. There shall be no consumption of wherever possible, providing that there is no adverse effect on
water or energy linked to their use, and they shall not cause the environment.
any emissions. The waste code in accordance with the European Waste Code
is 17 04 07.
2.11 Environment and health during use
2.16 Further information
No environmental damage or health risks are to be expected
during normal conditions of use. Details of all types and variants can be found on the
manufacturers' websites. The respective website addresses are
2.12 Reference service life available at https://arge.org.
3. LCA: Calculation rules
metals. When recycled metals are used as raw material only
3.1 Declared Unit
their transformation process is taken into account and not the
The declared unit for all products covered by ARGE EPD is 1 extraction of the raw material.
kg (of product). Since individual products will rarely weigh A4 module represents the transport of the finished door/window
exactly 1 kg it is necessary to establish the exact weight of the handle to the installation site.
product and then use this as a correction factor to determine There is no waste associated with the installation of the
the true values for 1 kg of product in the tables (Section 5). product. The A5 module therefore represents only the disposal
Declared unit of the product packaging.
The End-of-Life (EoL) stages are also considered. The
Name Value Unit
transportation to the EoL disposal site is taken into account in
Declared unit 1 kg
module C2. Module C4 covers the disposal of the locks. Module
Mass of declared product 0.749 kg C3 covers the recycling of the individual elements according to
Raw density 1 kg/m3 European averages, with the remaining waste divided between
incineration and landfill. Such a mixed scenario is declared due
to the complex material mix of the product and the dependency
of the EoL-route on the EoL-route of the product the
3.2 System boundary
door/window handle has been integrated into.
Type of the EPD: "cradle to gate with options, with modules C1
In practice, the end of life has been modelled as follows:
– C4, and module D (A1-A3, C1-C3, D and additional
modules)" • when a material is sent for recycling, generic transport
and electric consumption of a shredder is taken into
The analysis of the product life cycle includes the production account (corresponding to the process 'Grinding,
and transport of the raw materials, the manufacture of the metals'). Only then, is the material considered to have
product and the packaging materials which are declared in attained the 'end-of-waste' state.
modules A1-A3. • each type of waste is modelled as a transport to the
Losses during production are considered as waste and are sent treatment site with a distance of 30 km. Parts sent for
for recycling. No recycling processes are taken into account recycling include electricity consumption (grinding) and
except for transport and electricity consumption for grinding the a flow ('Materials for recycling, unspecified').
3 Environmental Product Declaration - ARGE – The European Federation of Locks and Building Hardware Manufacturers - Door and window handles
2022).
3.3 Estimates and assumptions • In the absence of collected data, generic data from the
The LCA data of the declared handle had been calculated by ecoinvent v3.8 database has been used. This is updated
the production data of a total of 3 ARGE member companies, regularly and is representative of current processes (the
collecting data on 11 different products. These companies had entire database having been updated in 2021).
been chosen by ARGE as being representative by means of Geography: Data come from production sites of the ARGE
their production processes and their market share. The handle member companies. Generic data come from the ecoinvent
chosen as representative for this calculation follows the "worst- database, representative for European production processes.
case" principle as explained under section 6. LCA
interpretation. Technology: Material shaping technologies are based on
European technology in the case of the use of generic data.
3.4 Cut-off criteria
The cut-off criteria considered are 1% of renewable and non- A total of 11 typical products (based on sales figures) have
renewable primary energy usage and 1% of the total mass of been evaluated and the worst-case results are used in section
that unit process. The total neglected input flows per module 5 of this EPD.
shall be a maximum of 5% of energy usage and mass.
3.7 Period under review
For this study, all input and output flows have been considered The data of the LCA is based on the annual production data of
at 100%, including raw materials as per the product an ARGE member company from 2013, considered also
composition provided by the manufacturer and packaging of representative for the year 2022.
raw materials as well as the final product. Energy and water
consumptions have also been considered at 100% according to 3.8 Geographic Representativeness
the data provided. Land or region, in which the declared product system is
manufactured, used or handled at the end of the product´s
With the approach chosen, no significant environmental lifespan: Europe
impacts are known to have been cut off.
3.5 Background data 3.9 Allocation
For the life cycle modelling of the considered product, all The products are produced in numerous production sites. All
relevant background datasets are taken from ecoinvent v3.8 data were provided by the manufacturers of the products per
(system model: cut-off by classification). unit and then divided by the mass of the product to give a value
per kg of product produced.
3.6 Data quality
The objective of this evaluation is to evaluate the environmental The assumptions relating to the EoL of the product are
impacts generated by the products throughout their entire life described in the section System Boundaries.
cycles. To this end, ISO 14040, ISO 14044 and EN 15804 have
been met regarding the quality of data on the following different 3.10 Comparability
criteria: Basically, a comparison or an evaluation of EPD data is only
possible if all the data sets to be compared were created
Time: The life cycle inventory data used come from: according to EN 15804 and the building context, respectively
the product-specific characteristics of performance, are taken
• Data collected specifically for this study on the ARGE
into account. ecoinvent v3.8 (system model: cut-off by
member companies' manufacturing sites. Datasets are
classification) has been used as the background database.
based on 1-year averaged data (time period: January
2013 to December 2013 considered representative for
4. LCA: Scenarios and additional technical information
Name Value Unit
Characteristic product properties of biogenic carbon
Material loss 0.137 kg
Information on the biogenic carbon content at factory gate
Note: 1 kg of biogenic carbon is equivalent to 44/12 kg of CO . Reference service life
2
Name Value Unit
Name Value Unit
Reference service life 30 a
kg
Biogenic carbon content in product 0 C Test cycles over RSL (EN 1906) 100'000 cycles
Biogenic carbon content in accompanying kg
0.342 End of life (C1-C4)
packaging C
Name Value Unit
Collected separately waste type 1 kg
The following information is the basis of the declared modules
Recycling 0.609 kg
within the LCA in this EPD.
Energy recovery 0.18 kg
Transport to the building site (A4)
Landfilling 0.211 kg
Name Value Unit
It is assumed that a 16–32-ton truck is used to transport the
Litres of fuel 25.8 l/100km
product:
Transport distance 3500 km
- Transport to shredding facility for metal recovery: 150 km
Capacity utilisation (including empty runs) 36 % - Transport to municipal waste incineration plant: 50 km
- Transport to landfill: 30 km
Installation into the building (A5)
4 Environmental Product Declaration - ARGE – The European Federation of Locks and Building Hardware Manufacturers - Door and window handles
Reuse, recovery and/or recycling potentials (D), relevant the corresponding amounts are declared as material for
scenario information recycling (MFR);
- net amounts of a metal leaving the product system are
Module D contains the benefits and loads beyond the system quantified as the material for recycling leaving modules A1-C4
boundary related to the recycling of metals, which result from minus the input of secondary scrap (secondary material, SM) to
the treatment of recycled materials from the point of end-of- the product system;
waste status to the point of substitution (as costs) and the - in the case of brass and zinc alloys, which are composed of
substitution of primary resources (as benefits). two different constituting metals, no difference shall be made
between the input of secondary constituting metals (Cu and Zn;
According to EN 16710, clause 6.4.3.3: 'In module D Cu and Sn) and its alloys (CuZn; CuSn).
substitution effects are calculated only for the resulting net
output flow. Negative net output flows have not been considered in the
quantification of module D.
For building hardware, the following rules apply for the
quantification of net output flows: It also includes the benefits and loads related to 'exported
- all production scrap and cuttings leave modules energy electricity' and 'exported energy heat' resulting from the
A1-B3 as sorted scrap without allocated burdens from primary energy recovery from plastic wastes in a municipal waste
production; incineration plant as modelled in Modules A3, A5 and C4.
5 Environmental Product Declaration - ARGE – The European Federation of Locks and Building Hardware Manufacturers - Door and window handles
5. LCA: Results
In Table 1 "Description of the system boundary", the declared modules are indicated with an "X"; all modules that are not declared
within the EPD but where additional data are available are indicated with "MND". Those data can also be used for building assessment
scenarios. The values are declared with three valid digits in exponential form.
The set of characterisation factors EF3.0 has been used for the life cycle assessment.
DESCRIPTION OF THE SYSTEM BOUNDARY (X = INCLUDED IN LCA; MND = MODULE OR INDICATOR NOT DECLARED; MNR
= MODULE NOT RELEVANT)
Benefits and
Construction loads beyond
Product stage Use stage End of life stage
process stage the system
boundaries
la ire wta am R y lp p u s tro p s n a rT g n iru tc a fu n a M tro p s nm ae o rh r
T
f te tis e h t o t e ta g y lb m e s s A e s U e c n a n e tn ia M ria p e R tn e m e c a lp e R tn e m h s ib ru fe R la n o ity ag rr ee pn Oe e s u la n o ita r re et pa Ow e s u n o itc u rts n eo Dc -n o itilo m e d tro p s n a rT g n is s ee tsc ao Wrp la s o p s iD e s u e R- y re v o c e R- g n ilc y c e R- la itn e to p
A1 A2 A3 A4 A5 B1 B2 B3 B4 B5 B6 B7 C1 C2 C3 C4 D
X X X X X MND MND MNR MNR MNR MND MND X X X X X
RESULTS OF THE LCA - ENVIRONMENTAL IMPACT according to EN 15804+A2: 1 kg of door or window handle
Parameter Unit A1-A3 A4 A5 C1 C2 C3 C4 D
GWP-total kg CO2 eq 6.47E+00 1.04E+00 1.29E+00 0 1.57E-02 3.37E-03 7.47E-03 -1.83E+00
GWP-fossil kg CO2 eq 7.71E+00 1.04E+00 3.86E-02 0 1.57E-02 3.37E-03 7.46E-03 -1.82E+00
GWP-biogenic kg CO2 eq -1.25E+00 0 1.25E+00 0 0 0 0 0
GWP-luluc kg CO2 eq 1.75E-02 4.16E-04 7.9E-06 0 6.26E-06 8.39E-06 3.64E-06 -3.64E-03
ODP kg CFC11 eq 6.38E-07 2.41E-07 4.55E-09 0 3.63E-09 1.71E-10 1.27E-09 -1.02E-07
AP mol H+ eq 3.94E-01 2.96E-03 6.43E-05 0 4.45E-05 1.73E-05 3.24E-05 -1.19E-01
EP-freshwater kg P eq 1.69E-03 7.42E-06 1.48E-07 0 1.12E-07 3.78E-07 6.38E-08 -5.29E-04
EP-marine kg N eq 2.19E-02 5.87E-04 1.54E-05 0 8.84E-06 2.22E-06 1.1E-05 -5.9E-03
EP-terrestrial mol N eq 4.31E-01 6.55E-03 1.7E-04 0 9.85E-05 2.57E-05 1.2E-04 -8.47E-02
kg NMVOC
POCP 7.65E-02 2.52E-03 5.85E-05 0 3.79E-05 7.03E-06 3.64E-05 -2.36E-02
eq
ADPE kg Sb eq 8.71E-03 3.69E-06 7.04E-08 0 5.55E-08 8.16E-09 1.43E-08 -2.93E-03
ADPF MJ 1.03E+02 1.58E+01 3E-01 0 2.37E-01 7.13E-02 9.48E-02 -2.22E+01
m3 world eq
WDP 6.94E+00 4.8E-02 1.06E-03 0 7.23E-04 7.97E-04 -4.06E-04 -2.08E+00
deprived
GWP = Global warming potential; ODP = Depletion potential of the stratospheric ozone layer; AP = Acidification potential of land and water; EP =
Eutrophication potential; POCP = Formation potential of tropospheric ozone photochemical oxidants; ADPE = Abiotic depletion potential for non-fossil
resources; ADPF = Abiotic depletion potential for fossil resources; WDP = Water (user) deprivation potential)
RESULTS OF THE LCA - INDICATORS TO DESCRIBE RESOURCE USE according to EN 15804+A2: 1 kg of door or window
handle
Parameter Unit A1-A3 A4 A5 C1 C2 C3 C4 D
PERE MJ 1.83E+01 2.22E-01 -7.05E-01 0 3.34E-03 1.35E-02 1.4E-03 -5.41E+00
PERM MJ 7.82E+00 0 -6.25E+00 0 0 0 0 0
PERT MJ 2.61E+01 2.22E-01 -6.96E+00 0 3.34E-03 1.35E-02 1.4E-03 -5.41E+00
PENRE MJ 1.03E+02 1.58E+01 5.72E-01 0 2.37E-01 7.2E-02 1.16E-01 -2.23E+01
PENRM MJ 3.18E-01 0 -2.71E-01 0 0 0 -2.12E-02 0
PENRT MJ 1.04E+02 1.58E+01 3E-01 0 2.37E-01 7.2E-02 9.48E-02 -2.23E+01
SM kg 5.43E-01 0 0 0 0 0 0 0
RSF MJ 0 0 0 0 0 0 0 0
NRSF MJ 0 0 0 0 0 0 0 0
FW m3 1.37E-01 1.67E-03 7.78E-05 0 2.52E-05 4.59E-05 1.99E-04 -3.63E-02
PERE = Use of renewable primary energy excluding renewable primary energy resources used as raw materials; PERM = Use of renewable primary
energy resources used as raw materials; PERT = Total use of renewable primary energy resources; PENRE = Use of non-renewable primary energy
excluding non-renewable primary energy resources used as raw materials; PENRM = Use of non-renewable primary energy resources used as raw
materials; PENRT = Total use of non-renewable primary energy resources; SM = Use of secondary material; RSF = Use of renewable secondary fuels;
NRSF = Use of non-renewable secondary fuels; FW = Use of net fresh water
RESULTS OF THE LCA – WASTE CATEGORIES AND OUTPUT FLOWS according to EN 15804+A2:
1 kg of door or window handle
Parameter Unit A1-A3 A4 A5 C1 C2 C3 C4 D
HWD kg 3.07E-03 4.12E-05 8.73E-07 0 6.2E-07 2.53E-08 1.8E-07 -8.41E-04
NHWD kg 3.67E+00 8.31E-01 1.65E-02 0 1.25E-02 2.68E-04 3.89E-01 -9.02E-01
RWD kg 7.68E-04 2.28E-04 4.27E-06 0 3.44E-06 9.59E-07 1.22E-06 -1.29E-04
CRU kg 0 0 0 0 0 0 0 0
MFR kg 8.48E-02 0 7.75E-01 0 0 5.04E-01 0 0
6 Environmental Product Declaration - ARGE – The European Federation of Locks and Building Hardware Manufacturers - Door and window handles
MER kg 0 0 0 0 0 0 0 0
EEE MJ 0 0 3.62E-02 0 0 0 9E-04 0
EET MJ 0 0 2.4E-01 0 0 0 5.96E-03 0
HWD = Hazardous waste disposed; NHWD = Non-hazardous waste disposed; RWD = Radioactive waste disposed; CRU = Components for re-use;
MFR = Materials for recycling; MER = Materials for energy recovery; EEE = Exported electrical energy; EET = Exported thermal energy
RESULTS OF THE LCA – additional impact categories according to EN 15804+A2-optional:
1 kg of door or window handle
Parameter Unit A1-A3 A4 A5 C1 C2 C3 C4 D
Disease
PM 1.29E-06 8.36E-08 1.64E-09 0 1.26E-09 4.63E-11 9.52E-10 -2.73E-07
incidence
IR kBq U235 eq 4.89E-01 6.85E-02 1.28E-03 0 1.03E-03 6.5E-04 3.65E-04 -9.99E-02
ETP-fw CTUe 2.96E+03 1.24E+01 2.43E-01 0 1.86E-01 3.59E-02 5.42E-01 -9.8E+02
HTP-c CTUh 7.16E-08 3.98E-10 9.7E-12 0 5.99E-12 9.59E-13 7E-12 -2.17E-08
HTP-nc CTUh 4.73E-06 1.25E-08 3.36E-10 0 1.88E-10 3.12E-11 8.35E-11 -1.55E-06
SQP SQP 1.7E+02 1.1E+01 2.06E-01 0 1.65E-01 1.1E-02 1.61E-01 -3.91E+01
PM = Potential incidence of disease due to PM emissions; IR = Potential Human exposure efficiency relative to U235; ETP-fw = Potential comparative
Toxic Unit for ecosystems; HTP-c = Potential comparative Toxic Unit for humans (cancerogenic); HTP-nc = Potential comparative Toxic Unit for humans
(not cancerogenic); SQP = Potential soil quality index
Disclaimer 1 –
for the indicator 'Potential Human exposure efficiency relative to U235'. This impact category deals mainly with the eventual impact of
low-dose ionizing radiation on human health of the nuclear fuel cycle. It does not consider effects due to possible nuclear accidents,
occupational exposure or radioactive waste disposal in underground facilities. Potential ionizing radiation from the soil, radon and from
some construction materials is also not measured by this indicator.
Disclaimer 2 –
for the indicators 'abiotic depletion potential for non-fossil resources', 'abiotic depletion potential for fossil resources', 'water (user)
deprivation potential, deprivation-weighted water consumption', 'potential comparative toxic unit for ecosystems', 'potential comparative
toxic unit for humans – cancerogenic', 'Potential comparative toxic unit for humans - not cancerogenic', 'potential soil quality index'. The
results of this environmental impact indicator shall be used with care as the uncertainties on these results are high as there is limited
experience with the indicator.
6. LCA: Interpretation
Figure 1 illustrates the relative contributions of the different
modules along the life cycle of the declared products.
Figure 1: Environmental impacts of door and window All the other modules related to the product life cycle are not
handles along its life cycle significant.
The largest part of environmental impacts is caused during Benefits and burdens beyond the system boundary (module D)
production (modules A1-A3); comparably small impacts are are in the order of 10 % to 25 % of the impacts over the product
caused during the transport of the product to the construction life cycle (modules A1-A3) and relate basically to the recycling
site (via the manufacturer of the product, which the of metals.
door/window handle has been integrated into).
7 Environmental Product Declaration - ARGE – The European Federation of Locks and Building Hardware Manufacturers - Door and window handles
A total of 11 typical products (based on sales figures) have weight per material ensures that the variability of results stays
been evaluated and the worst-case results are used in section within +/- 40% of the declared values (assessed for the
5 of this EPD. In chapter 2.5, the tabulated range of relative indicators GWP, PENRT, and non-hazardous waste).
7. Requisite evidence
No testing results are required by the PCR part B.
8. References
Product category rules of IBU furniture - Requirements and test methods.
IBU (2021) EN 13126
IBU (2021): General Instructions for the EPD Programme of the EN 13126-3:2023, Building hardware - Hardware for windows
Institut Bauen und Umwelt e.V. (General Instructions for the and door-height windows - Requirements and test methods -
IBU EPD Programme). Version 2.0, Institut Bauen und Umwelt, Part 3: Handles, primarily for Tilt and Turn, Tilt-First and Turn-
Berlin. Only hardware.
IBU (2021) ISO 15686
IBU (2021): PCR Part A: Calculation rules for the life cycle ISO 15686:1, -2, -7 and -8. Service life planning (various parts).
assessment and requirements on the project report according
to EN 15804+A2. Version 1.3., Institut Bauen und Umwelt, ECHA candidate list
Berlin. Candidate List of substances of very high concern for
Authorisation, published in accordance with Article 59(10) of the
IBU (2023) REACH Regulation. European Chemicals Agency, Brussels.
IBU (2023): PCR Part B: Requirements on the EPD for building
hardware products, Institut Bauen und Umwelt, Berlin. Ordinance on Biocide Products No. 528/2012
REGULATION (EU) No 528/2012 OF THE EUROPEAN
Standards and legal documents PARLIAMENT AND OF THE COUNCIL of 22 May 2012
concerning the making available on the market and use of
EN 15804 biocidal products.
EN 15804:2012+A2:2019+AC:2021, Sustainability of
construction works - Environmental product declarations - Core European List of Waste
rules for the product category of construction products. Commission Decision of 3 May 2000 replacing Decision
94/3/EC establishing a list of wastes pursuant to Article 1(a) of
EN 17610 Council Directive 75/442/EEC on waste and Council Decision
EN 17610:2022, Building hardware - Environmental product 94/904/EC establishing a list of hazardous waste pursuant to
declarations - Product category rules complementary to EN Article 1(4) of Council Directive 91/689/EEC on hazardous
15804 for building hardware. waste (notified under document number C(2000) 1147).
ISO 14025 Additional references
ISO 14025:2006-07, Environmental labels and declarations -
Type III Environmental declarations - Principles and BBSR 2017
procedures. BBSR (2017): Nutzungsdauer von Bauteilen in
Lebenszyklusanalysen nach Bewertungssystem Nachhaltiges
ISO 14044 Bauen (BNB). Version vom 24.10.2017, Bundesinstitut für Bau-,
EN ISO 14044:2006, Environmental management - Life cycle Stadt- und Raumforschung, Berlin.
assessment - Requirements and guidance (ISO 14044:2006).
ecoinvent v3.8
EN 1906 http://www.ecoinvent.org
EN 1906:2012, Building hardware - Lever handles and knob
8 Environmental Product Declaration - ARGE – The European Federation of Locks and Building Hardware Manufacturers - Door and window handles
Publisher
Institut Bauen und Umwelt e.V. +49 (0)30 3087748- 0
Hegelplatz 1 info@ibu-epd.com
10117 Berlin www.ibu-epd.com
Germany
Programme holder
Institut Bauen und Umwelt e.V. +49 (0)30 3087748- 0
Hegelplatz 1 info@ibu-epd.com
10117 Berlin www.ibu-epd.com
Germany
Author of the Life Cycle Assessment
Dr. Frank Werner - Umwelt & Entwicklung + 41 (0)44 241 39 06
Kammelenbergstrasse 30 frank@frankwerner.ch
9011 St. Gallen http://www.frankwerner.ch/
Switzerland
Owner of the Declaration
ARGE – The European Federation of Locks and +49 (0)2051 9506 15
Building Hardware Manufacturers mail@arge.org
Offerstraße 12 www.arge.org
42551 Velbert
Germany
9 Environmental Product Declaration - ARGE – The European Federation of Locks and Building Hardware Manufacturers - Door and window handles
