ENVIRONMENTAL-PRODUCT DECLARATION
as per ISO 14025 and EN 15804+A1
Owner of the Declaration Grundfos Holding A/S
Publisher Institut Bauen und Umwelt e.V. (IBU)
Programme holder Institut Bauen und Umwelt e.V. (IBU)
Declaration number EPD-GRU-20200112-CCC1-EN
Issue date 24.02.2021
Valid to 23.02.2026
UPM3 (Composite)
Grundfos Holding A/S
www.ibu-epd.com | https://epd-online.com
General Information
Grundfos Holding A/S UPM3 (Composite)
Programme holder Owner of the declaration
IBU – Institut Bauen und Umwelt e.V. Grundfos Holding A/S
Hegelplatz 1 Poul Due Jensens Vej 7
10117 Berlin 8850 Bjerringbro
Germany Denmark
Declaration number Declared product / declared unit
EPD-GRU-20200112-CCC1-EN 1 PCS. of UPM3 (Composite)
This declaration is based on the product category rules: Scope:
Pumps for liquids and liquids with solids, 01.08.2021 The declaration applies to 1 piece of UPM3 (Composite) pump. The
(PCR checked and approved by the SVR) product is produced in Longeville -Les -Saint Avold, France, and the life
cycle assessment is based on data collected at the production site.
Production has been modeled using annual
Issue date production data
from 2019.
24.02.2021
The declaration covers whole range of UPM3 (Composite) pump.
Valid to
The owner of the declaration shall be liable for the underlying information
23.02.2026 and evidence; the IBU shall not be liable with respect to manufacturer
information, life cycle assessment data and evidences.
The EPD was created according to the specifications of EN 15804+A1. In
the following, the standard will be simplified as EN 15804 bezeichnet.
Verification
The standard EN 15804 serves as the core PCR
Independent verification of the declaration and data according to ISO
14025:2011
internally X externally
Dipl.-Ing Hans Peters
(chairman of Institut Bauen und Umwelt e.V.)
Dr. Alexander Röder Dr. Patricia Wolf,
(Managing Director Institut Bauen und Umwelt e.V.) (Independent verifier)
1 Environmental-Product Declaration - Grundfos Holding A/S - UPM3 (Composite)
Product
Product description/Product definition
The Grundfos UPM3 pumps are of the canned-rotor type as
pump and motor form an integral unit without shaft seal and
with only one gasket for sealing and four screws for fastening
the stator housing to the pump housing. The bearings are The UPM3 range is designed for all kinds of Heating,
lubricated by the pumped liquid as the rotor can is filled with Ventilation and Air-Conditioning applications:
media.
The basic UPM3 hardware model is controlled via a signal
cable entry (e.g. PWM or LINBUS) and does not feature a user
interface. The UPM3 Hybrid, on the other hand, combines
external signal controlling and internal self-controlling. • Boiler systems
The declaration covers whole range of the UPM3 (Composite)
pump. They are grouped as shown below.
• Heat pumps
GROUP 1 - UPM3S
GROUP 2 - UPM3 and UPM3L
More information about UPM3 • Solar thermal systems
(Composite) variants can be
found in Grundfos data booklet.
• Heating kits
• Domestic hot water systems
For the placing on the market in the EU/EFTA (with the • Micro combined heat and power systems.
exception of Switzerland) the following legal provisions apply:
Technical Data
The performance data of the product according to the
harmonised norms, based on the harmonisation provisions
above apply.
Low Voltage Directive
(2014/35/EU)
Standards used: EN
603351:2012A11:2014/A13:20, EN 60335-2-51:2003 A1:2008
A2:2012.
EMC Directive (2014/30/EU) The relevant technical specifications according to the PCR Part
Standards used: EN 55014-1:2017, EN B is given in the table below.
55014-2:2015, EN 61000-3-2:2014/2019, EN 61000-6- Note:
2:2008/2019, EN Electrical pumps usually falls under the scope of several
61000-3-3:2013 A1:2019. internal market
RoHS Directive 2011/65/EU and 2015/863//EU directives and regulations, such as the Machinery directive,
Standard: EN 50581:2012 Ecodesign
Ecodesign Directive (2009/125/EC) Directive, Radio Equipment Directive etc. The relevant technical
Commission Regulation (EC) No 641/2009 data given in
Commission Regulation (EC) No 622/2012 the EPD will vary depending on the type of product and areas
Standards used: EN 16297-1:2012, EN of application,
16297-2:2012, EN 16297-3:2012. and the table below should be adjusted accordingly.
EEI ≤ 0.20 is stated according to EN 16297. The CE-marking
Constructional data
takes into account the proof
of conformity with the respective harmonized norms based on
the legal
provisions above.
For
the application and use the respective national provisions apply.
UPM3 pump is
not harmonized in accordance with the CPR.
Application
The Grundfos UPM3 pumps are designed for heating, cooling
and domestic hot water applications and can be configures in
different variants suitable for each application. On the
production side there are some applications where pumps are
used in primary or internal circuits e.g. for geothermal or solar
thermal brine circuits.
2 Environmental-Product Declaration - Grundfos Holding A/S - UPM3 (Composite)
Name Value Unit
Frequency 50/60 Hz
REACH
Flow range Gr.1, UPM3S (max) 2,25 m3/h
Flow range Gr.2, UPM3 (max) 2,8 m3/h
Flow range Gr.2, UPM3L (max) 2,5 m3/h This product/article/at least one partial article contains
substances listed in the ECHA candidate list (date: 27.06.2018)
Head max Gr.1, UPM3S 6,0 m
exceeding 0.1 percentage by mass: no
Head max Gr.2, UPM3 7,5 m
Head max Gr.2, UPM3L 7,5 m
Average power consumption Gr.1, UPM3S
0,018 kW
(based on EN16297-1)
Average power consumption Gr.2, UPM3
0,025 kW
(based on EN16297-1) ISO 14001
Average power consumption Gr.2, UPM3L
0,022 kW
(based on EN16297-1)
Production at Longeville-Les-Saint Avold in France has been
Nominal power consumption Gr.1, UPM3S
0,042 kW assessed and certified as meeting the requirements in ISO
(max)
14001:2015.
Nominal power consumption Gr.2, UPM3
0,06 kW
(max) Environment and health during use
Nominal power consumption Gr.2, UPM3L
0,06 kW Reference service life
(max)
No use stage scenario which refers to the lifetime of the product
230 (-15% to
Voltage V is declared. Product lifetime is calculated based on the
+10%)
assessed weakest part to be 12 years in average. Calculation
Energy efficiency Index 0,20
is based on performance test, knowledge of load profile and
Pumped liquid (e.g. water) Water and equations provided by component supplier. Assessment is
Glycol based on expert opinion.
Performance data of Service life of the declared product is not directly influencing
the product according to the harmonised standards, based on the results in this study, as no declared use stage scenario is
provisions for dependent on the service life. The use stage sub-module B6 is
harmonization. declared per year as required by the PCR Part B.
Base materials/Ancillary materials
Name Value Unit
Aluminium 11,5 %
Cardboard 8,7 %
Ceramics 1,3 %
Copper 10,6 %
Magnet 1,4 %
Electronics 1,4 %
Plastic film 0,2 %
Plastics 1,1 %
Plastics GF 24,9 %
Rubber 0,7 %
Stainless steel 10,9 %
Steel 16,1 %
Wood pallet 11,2 %
TOTAL 100 %
LCA: Calculation rules
production process, geographical representativeness and the
Declared Unit influence of background data and preliminary products
The declared unit refers to 1 piece of UPM3 (Composite) pump. compared to the environmental impacts caused by actual
production.
For the LCA calculations is used average mass reference
(based on product groups).
System boundary
Declared unit
This EPD is
Name Value Unit
Cradle-To-Grave.The system boundaries of the EPD follow the
Declared unit 1 pce. modular approach in EN 15804.
Mass reference 1,54 kg/pce. By decision no.
20170712-n of the SVR, the modules B3, B4 and B5 are by
For IBU core EPDs (where clause 3.6 is part of the EPD): for
default declared
average EPDs, an estimate of the robustness of the LCA
as "MNR" (module not relevant).
values must be made, e.g. concerning variability of the
3 Environmental-Product Declaration - Grundfos Holding A/S - UPM3 (Composite)
Waste for incineration arising in the product stage is accounted
for in the module where the waste is produced. The
environmental loads from the incineration process are declared
in the module where it occurs and the electricity and heat which
is produced from the incineration is considered as closed-loop
within A1-A3, as described in PCR Part A, 5.5.1. Input of
biogenic carbon from the production of packaging material is
inventoried in A3. As required by PCR Part A, the
corresponding end-of-life module of the packaging material, A5,
is also declared and the emissions of biogenic carbon
inventoried.
The product stage (A1-A3) comprises raw material extraction
and processing, transport processes as well as the
manufacturing process. The product stage is included in the The construction process stage (A4-A5) includes:
study, and according to /EN 15804/ the system boundary with
nature is set to include those processes that provide the
material and energy inputs into the system and the following A4:
manufacturing, transport up to the factory gate as well as the
processing of any waste arising from those processes.
• Transportation from factory gate to distribution center
Wastes and losses are included in the modules where they
• Consumption of electricity, thermal energy and water at
occur according to the polluter pays principle and the modular
distribution center
approach of EN 15804.
• Transportation from distribution center to construction
site
• Wastage during distribution
A5:
The product stage includes:
• Installation process
• Transport of packaging waste to treatment site
• A1 Extraction and processing of raw materials;
• Waste treatment of packaging
• A1 Reuse of products or materials from a previous
product system;
• A1 Processing of secondary materials;
• A1 Generation of electricity, steam and heat from
primary energy resources, also including their
extraction, refining and transport;
The packaging material does not reach the end of waste state
• A1 Energy recovery and other recovery processes from
but is incinerated as waste. According to European statistics,
secondary fuels;
the average R1 value of incineration plants is > 0.6. Therefore,
• A2 Transportation up to the factory gate and internal
it is assumed that packaging material are treated thermally in
transport;
an incineration plant with R1 > 0.6. The loads from the
• A3 Production of ancillary materials or pre - products;
combustion process of packaging are declared in module A5
• A3 Manufacturing of products and coproducts;
and the resulting energy benefits in module D, as required by
• A3 Manufacturing of packaging;
the PCR Part A, 5.5.2.
• A1-A3 processing up to the end-of-waste state or
disposal of final residues.
For secondary material inputs, the system boundary to the
Use stage (B1-B7):
previous system (providing the secondary material) is set where
outputs reach the end-of-waste state. The recycling of
secondary material into new raw materials is included in the
system boundary of this study. Waste materials from production
processes that is recycled without any modification of the
material inherent characteristics are modelled as closed loop
The use stage, related to the building fabric includes:
within A1-A3. This is done up to the input mass flow that was
used during production.
• B1, use or application of the installed product
• B2, maintenance
4 Environmental-Product Declaration - Grundfos Holding A/S - UPM3 (Composite)
management of the disposal site
The use stage related to the operation of the building includes:
• B6, operational energy use
At end of life, the UPM3 pump is manually disassembled from
• B7, operational water use
the piping system in which it has been installed. The definition
of the applied end-of-life scenario in this EPD follows the
requirements in the PCR Part A, 6.2 regarding complex
products, with a combination of recycling, thermal waste
treatment and landfilling. 100 % of the material is considered in
the end of life scenario as required by the PCR. An overall
In this study, all use stage modules are assessed, though B1,
collection rate of 90 % have been assumed.
B2 and B7 are assessed to be zero. By decision no. 20170712-
n of the SVR, the modules B3, B4 and B5 are by default
Materials from which energy is recovered in an incineration
declared as "MNR" (module not relevant). The modules include
process with a R1-value above 0.60 are in this study included
the provision and transport of all materials, products and
with the environmental burdens from the incineration process
related energy and water use, as well as waste processing up
inventoried in C3, the recovered energy is declared as exported
to the end-of-waste state or disposal of final residues during the
energy in C3 and the energy benefits is declared in D. This
use stage. They also include all impacts and aspects related to
procedure is according to the PCR Part A, 5.5.6. C3 includes
the losses during the use stage (i.e. production, transport, and
the mechanical separation of the product followed by a series
waste processing and disposal of the lost products and
of sorting steps. Metal fractions are recycled and plastics,
materials).
cardboard and electronics are assumed incinerated with energy
recovery. The residual fractions are landfilled and declared in
C4. The specific amounts are shown in the scenarios section.
Beyond system boundary (D): According to /EN 15804/
Contributions to operational energy use during the use stage
module D includes the reuse, recovery and/or recycling
(B6) comes from the electricity consumption of the product. The
potentials, expressed as net impacts and benefits. Any
annual electricity consumption is calculated by multiplying the
declared benefits and loads from net flows leaving the product
average power input, which is based on a defined load profile,
system that have not been allocated as co-products and that
with the annual running hours. These values are declared in the
have passed the end-of-waste state are included in module D.
scenarios section.
Contributions to module D comes from waste incineration
processes in A5 and C3 as well as material recycling in C3. The
specific fractions and net flows are shown in the scenarios
section.
The End-of-Life stage (C1-C4) includes all activities from
when the product reaches the end of its service life and no
longer provides any functionality and until all materials and
components are processed for reuse/recycling or disposed of.
According to EN 15804 and the PCR Part A, the end of life
stage includes:
Geographic Representativeness
Land or region, in which the declared product system is
manufactured, used or handled at the end of the product´s
• C1 deconstruction of the product from the building, lifespan: France
including initial on-site sorting of the materials
• C2 transportation of the discarded product to a recycling
site and transportation of waste to final disposal Comparability
• C3 waste processing, collection of waste fractions from Basically, a comparison or an evaluation of EPD data is only
the deconstruction and waste possible if all the data sets to be compared were created
• processing of material flows intended for reuse, according to EN 15804 and the building context, respectively
recycling and energy recovery the product-specific characteristics of performance, are taken
• C4 waste disposal including physical pretreatment and into account.
LCA: Scenarios and additional technical information
Name Value Unit
The following technical information forms the basis for the
Litres of fuel 0,0129 l/100km
declared gate-to-grave modules and can be used for
Transport distance 1000 km
developing specific scenarios in the context of a building
Capacity utilisation (including empty runs) 85 %
assessment.
Gross density of products transported 103 kg/m3
Transport from the gate to the site (A4)
Wastage during distribution 0,01 %
Installation into the building (A5)
5 Environmental-Product Declaration - Grundfos Holding A/S - UPM3 (Composite)
Name Value Unit End of life (C1-C4)
Packaging waste for incineration (PE film) 0,00405 kg
Name Value Unit
Packaging waste for incineration (Wood pallet) 0,172 kg
Collected as mixed construction waste 1,23 kg
Packaging waste for incineration (Cardboard) 0,134 kg
Transportation distance (C2) 500 km
Service life is calculated based on the assessed weakest part Aluminium for recycling 0,179 kg
to be 12 years in average. Calculation is based on performance Steel for recycling 0,215 kg
test, knowledge of load profile and equations provided by
Copper for recycling 0,131 kg
component supplier. Assessment is based on expert opinion.
Stainless steel for recycling 0,147 kg
Reference service life
Cardboard for incineration w/energy 0,134 kg
Name Value Unit
Plastics for incineration w/energy 0,361 kg
Life Span according to the manufacturer 12 a
Electronics for incineration w/energy 0,0194 kg
Operational energy use (B6) Landfilling 0,15 kg
Reuse, recovery and/or recycling potentials (D), relevant
Name Value Unit scenario information
Electricity consumption Gr.1, UPM3S 196,87kWh/a The values in the table are flow amounts which contributes to
Electricity consumption Gr.2, UPM3 281,25kWh/a module D.
Electricity consumption Gr.2, UPM3L 281,25kWh/a Name Value Unit
Average power consumption Gr.1, UPM3S A5, incineration w/energy recov. (PE foil) 0,00405 kg
0,018 kW
(based on EN16297-1) A5, incineration w/energy recov. (Wood pallet) 0,172 kg
Average power consumption Gr.2, UPM3 (based A5, incineration w/energy recov. (Cardboard) 0,134 kg
0,025 kW
on EN16297-1)
C3, steel for recycling (net amounts) 0,116 kg
Average power consumption Gr.2, UPM3L
0,022 kW C3, stainless steel for recycling (net amounts) 0,114 kg
(based on EN16297-1)
Running hours (all groups) 8760 h/a
6 Environmental-Product Declaration - Grundfos Holding A/S - UPM3 (Composite)
LCA: Results
Characterization
model: CML 2001 – January, 2016. The LCA results in B6 refers to a period of
one year, as required by the PCR Part B. To quantify B6 over the total life
cycle, the LCA results of module B6 is multiplied by 12 (estimated service
life).
The indicator results for module B6 are declared for UPM3S.
B6 indicator results for UPM3
and UPM3L can be derived by multiplying the B6 indicator results with the
following factor:
UPM3 and UPM3L: 1,71
DESCRIPTION OF THE SYSTEM BOUNDARY (X = INCLUDED IN LCA; MND = MODULE NOT DECLARED; MNR = MODULE NOT
RELEVANT)
BENEFITS
AND LOADS
CONSTRUCTION
BEYOND
PRODUCT STAGE PROCESS USE STAGE END OF LIFE STAGE
THE SYSTEM
STAGE
BOUNDARIE
S
la ire ta m w a Ry lp p u s tro p s n a rT g n iru tc a fu n a M e h t m o rf tro p s n a rTe tis e h t o t e ta g y lb m e s s A e s U e c n a n e tn ia M ria p e R tn e m e c a lp e R tn e m h s ib ru fe R y g re n e la n o ita re p Oe s u re ta w la n o ita re p Oe s u n o itc u rts n o c -e Dn o itilo m e d tro p s n a rT g n is s e c o rp e ts a W la s o p s iD -e s u e R-y re v o c e R-g n ilc y c e Rla itn e to p
A1 A2 A3 A4 A5 B1 B2 B3 B4 B5 B6 B7 C1 C2 C3 C4 D
X X X X X X X MNR MNR MNR X X X X X X X
RESULTS OF THE LCA - ENVIRONMENTAL IMPACT according to EN 15804+A1: 1 PCS of UPM3S (Composite)
Parameter Unit A1-A3 A4 A5 B1 B2 B6 B7 C1 C2 C3 C4 D
GWP kg CO 2 eq 1.64E+01 1.01E-01 5.12E-01 0 0 6.48E+01 0 0 3.35E-02 1.14E+00 8.81E-03 -1.22E+00
kg CFC11
ODP 8.76E-08 1.76E-11 1E-16 0 0 1.94E-12 0 0 8.39E-18 3.76E-15 2.89E-17 -1.39E-14
eq
AP kg SO 2 eq 1.47E-01 2E-04 7.46E-05 0 0 1.36E-01 0 0 1.38E-04 3.24E-04 2.47E-05 -6.29E-03
EP kg PO 43 eq 8.44E-02 5.49E-05 1.49E-05 0 0 1.5E-02 0 0 3.46E-05 4.49E-05 1.62E-05 -3.1E-04
kg Ethen
POCP 7.8E-03 -3.68E-05 3.55E-06 0 0 9.68E-03 0 0 -5.67E-05 2.47E-05 2.57E-06 -4.08E-04
eq
ADPE kg Sb eq 4.91E-03 1E-06 7.44E-09 0 0 2.16E-05 0 0 3.1E-09 4.89E-08 1.73E-09 -1.43E-04
ADPF MJ 2.15E+02 1.35E+00 1.25E-01 0 0 7.18E+02 0 0 4.57E-01 1.49E+00 1.34E-01 -1.42E+01
GWP = Global warming potential; ODP = Depletion potential of the stratospheric ozone layer; AP = Acidification potential of land and water; EP =
Eutrophication potential; POCP = Formation potential of tropospheric ozone photochemical oxidants; ADPE = Abiotic depletion potential for non-fossil
resources; ADPF = Abiotic depletion potential for fossil resources
RESULTS OF THE LCA - INDICATORS TO DESCRIBE RESOURCE USE according to EN 15804+A1: 1 PCS of UPM3S
(Composite)
Parameter Unit A1-A3 A4 A5 B1 B2 B6 B7 C1 C2 C3 C4 D
PERE MJ 4.14E+01 1.32E-01 5.2E+00 0 0 0 0 0 0 9.6E+00 9.69E-03 -2.09E+00
PERM MJ 5.2E+00 0 -5.18E+00 0 0 0 0 0 0 -8.61E+00 0 0
PERT MJ 4.14E+01 1.32E-01 2.49E-02 0 0 5.15E+02 0 0 2.64E-02 9.96E-01 9.69E-03 -2.09E+00
PENRE MJ 2.49E+02 1.42E+00 3.2E-01 0 0 0 0 0 0 1.1E+01 1.38E-01 -1.6E+01
PENRM MJ 1.02E+01 0 -1.7E-01 0 0 0 0 0 0 -8.61E+00 0 0
PENRT MJ 2.49E+02 1.42E+00 1.43E-01 0 0 1.16E+03 0 0 4.59E-01 2.35E+00 1.38E-01 -1.6E+01
SM kg 5.38E-01 1.08E-04 0 0 0 0 0 0 0 0 0 0
RSF MJ 2.53E-25 5.09E-29 0 0 0 0 0 0 0 0 0 0
NRSF MJ 2.98E-24 5.98E-28 0 0 0 0 0 0 0 0 0 0
FW m3 1.24E-01 1.85E-04 1.34E-01 0 0 5.95E-01 0 0 3.08E-05 3.17E-03 1.76E-06 -4.2E-03
PERE = Use of renewable primary energy excluding renewable primary energy resources used as raw materials; PERM = Use of renewable primary
energy resources used as raw materials; PERT = Total use of renewable primary energy resources; PENRE = Use of non-renewable primary energy
excluding non-renewable primary energy resources used as raw materials; PENRM = Use of non-renewable primary energy resources used as raw
materials; PENRT = Total use of non-renewable primary energy resources; SM = Use of secondary material; RSF = Use of renewable secondary fuels;
NRSF = Use of non-renewable secondary fuels; FW = Use of net fresh water
RESULTS OF THE LCA – WASTE CATEGORIES AND OUTPUT FLOWS according to EN 15804+A1:
1 PCS of UPM3S (Composite)
Parameter Unit A1-A3 A4 A5 B1 B2 B6 B7 C1 C2 C3 C4 D
HWD kg 1.23E-06 5.75E-08 7.27E-10 0 0 8.63E-07 0 0 2.12E-08 1.13E-09 5.53E-10 -7.09E-05
NHWD kg 9.12E-01 4.6E-04 9.14E-03 0 0 1.48E+00 0 0 7.28E-05 3.27E-02 1.58E-01 1.06E-01
RWD kg 1.3E-02 2.6E-05 7.16E-06 0 0 3.16E-01 0 0 8.46E-07 3.4E-04 1.65E-06 -7.18E-04
7 Environmental-Product Declaration - Grundfos Holding A/S - UPM3 (Composite)
CRU kg 0 0 0 0 0 0 0 0 0 0 0 0
MFR kg 0 0 0 0 0 0 0 0 0 6.71E-01 0 0
MER kg 0 0 0 0 0 0 0 0 0 0 0 0
EEE MJ 0 0 7.58E-01 0 0 0 0 0 0 1.64E+00 0 0
EET MJ 0 0 1.37E+00 0 0 0 0 0 0 2.94E+00 0 0
HWD = Hazardous waste disposed; NHWD = Non-hazardous waste disposed; RWD = Radioactive waste disposed; CRU = Components for re-use;
MFR = Materials for recycling; MER = Materials for energy recovery; EEE = Exported electrical energy; EET = Exported thermal energy
Note: The use of secondary material (SM) in A4 comes from product wastage during distribution.
References
PCR Part A
EN
55014-2:2015 Electromagnetic compatibility – Requirements for
Institut Bauen und Umwelt e.V., Berlin (pub.): Product household
Category Rules for Building-Related Products and Services, appliances, electric tools and similar apparatus – Part 2:
Product Category Rules for Construction Products from the Immunity – Product
range of family standard (CISPR 14-2:2015)
Environmental Product Declarations of Institut Bauen und
Umwelt (IBU), Part
A: Calculation Rules for the Life Cycle Assessment and
Requirements
on the Project Report, Version 1.7 (2018)
Electromagnetic
Compatibility (EMC) Directive
PCR Part B DIRECTIVE
2014/30/EU OF THE EUROPEAN PARLIAMENT AND OF THE
COUNCIL of 26 February 2014 on
the harmonisation of the laws of the Member States relating to
Institut Bauen und Umwelt e.V., Berlin (pub.): Product Category electromagnetic
Rules for Building-Related Products and Services, Product compatibility
Category Rules for Construction Products from the range of
Environmental
Product Declarations of Institut Bauen und Umwelt (IBU), Part
B: Requirements on the EPD for Pumps for liquids and liquids
with
solids, Version 1.0(2018)
DIRECTIVE
2011/65/EU
DIRECTIVE
IBU 2016 2011/65/EU OF THE EUROPEAN PARLIAMENT AND OF THE
COUNCIL of 8 June 2011 on
the restriction of the use of certain hazardous substances in
electrical and
IBU (2016): electronic equipment
General Programme Instructions for the Preparation of EPDs at
the Institut
Bauen und Umwelt e.V., Version 1.1 Institut Bauen und Umwelt
e.V.,Berlin.
www.ibu-epd.de DIRECTIVE
2015/863/EU
EN 55014-2 DIRECTIVE
2015/863/EU of 31 March 2015 amending Annex II to Directive
8 Environmental-Product Declaration - Grundfos Holding A/S - UPM3 (Composite)
2011/65/EU of 61000-6-2:2008/2019 Electromagnetic compatibility (EMC) –
the European Parliament and of the Council as regards the list Part 6-2: Generic
of restricted standards – Immunity for industrial environments
substances
EN 61000-3-2
EN 50581:2012 EN
61000-3-2:2014/2019 Electromagnetic compatibility (EMC) –
Part 3-2: Limits –
Limits for harmonic current emissions (equipment input current
EN = 16 A per
50581:2012 Technical documentation for the assessment of phase)
electrical and
electronic products with respect to the restriction of hazardous
substances
EN 61000-3-3
EN 61000-3-3:2013-08/
A1:2019 Electromagnetic compatibility (EMC) – Part 3-3: Limits
EN 60335-1 – Limitation of
voltage changes, voltage fluctuations and flicker in public low
voltage supply
systems, for equipment with rated current <= 16 A per phase
EN and not subject
60335-1:2012/A11:2014/A13:2017 - Household and similar to conditional connection
electrical appliances –
Safety – Part 1: General requirements
EN 60335-2-51
Ecodesign
Directive
EN
60335-2-51:2003-03 + A1:2008 + A2:2012 Household and
similar electrical DIRECTIVE
appliances – Safety – Part 2-51: Particular requirements for 2009/125/EC OF THE EUROPEAN PARLIAMENT AND OF
stationary THE COUNCIL of 21 October 2009
circulation pumps for heating and service water installations establishing a framework for the setting of ecodesign
requirements for
energy-related products
EN 55014-1
EC 641/2009
EN 55014-1:2017
Electromagnetic compatibility – Requirements for household
appliances, electric COMMISSION
tools and similar apparatus – Part 1: Emission REGULATION (EC) No 641/2009 of 22 July 2009 implementing
Directive 2005/32/EC
of the European Parliament and of the Council with regard to
ecodesign
requirements for glandless standalone circulators and
EN 61000-6-2 glandless circulators
integrated in products
EN
9 Environmental-Product Declaration - Grundfos Holding A/S - UPM3 (Composite)
EC 622/2012
CPR
COMMISSION REGULATION
(EU) No 622/2012 of 11 July 2012 amending Regulation (EC)
No 641/2009 with REGULATION (EU)
regard to ecodesign requirements for glandless standalone No 305/2011 OF THE EUROPEAN PARLIAMENT AND OF
circulators and THE COUNCIL of 9 March 2011
glandless circulators integrated in products laying down harmonised conditions for the marketing of
construction products
and repealing Council Directive 89/106/EEC
EN 16297-1
GaBi ts
EN
16297-1:2012-10 Pumps – Rotodynamic pumps –Glandless
circulators – Part 1: GaBi ts 9.2.1.68 (database schema 8007)
General requirements and procedures for testing and
calculation of energy
efficiency index (EEI)
Ecoinvent
EN 16297-2
Ecoinvent v3.5
EN
16297-2:2012-10 Pumps – Rotodynamic pumps –Glandless
circulators – Part 2:
Calculation of energy efficiency index (EEI) for standalone
circulators
CML
2001
Impact
assessment characterization factors
EN 16297-3
Institute
EN 16297-3:2012 Pumps of Environmental Sciences, Leiden University, Netherlands
– Rotodynamic pumps – Glandless circulators – Part 3: Energy
efficiency index
(EEI) for circulators integrated in products
SVR
ISO 14001
Advisory
Board (formerly SVA)
EN ISO
14001:2015-09 Environmental management systems -
Requirements with guidance for Decision
use no. 20170712-n
10 Environmental-Product Declaration - Grundfos Holding A/S - UPM3 (Composite)
concerning the Registration, Evaluation, Authorisation
ISO 14025
and Restriction of Chemicals (REACH)
(Status: 27.06.2018)
DIN EN /ISO
14025:2011-10/, Environmental labels
ECHA candidate list
and
declarations — Type III environmental declarations —
Principles and procedures Candidate List of substances of very high concern
(SVHCs) for authorisation, European
EN 15804
EN
15804:2012-04+A1 2013/, Sustainability of construction works
— Environmental Chemicals Agency (ECHA),
Product Declarations — Core rules for the product category of Helsinki, Finland
construction
products
REACH
Regulation (EC) No 1907/2006 of the European
The literature referred to in the Environmental Product
Parliament and of the Council of 18 December 2006 Declaration must be listed in full.Standards already fully quoted
in the EPD do not need to be listed here again.
The current version of PCR Part A and PCR Part B of the PCR
document on which they are based must be referenced.
11 Environmental-Product Declaration - Grundfos Holding A/S - UPM3 (Composite)
Publisher
Institut Bauen und Umwelt e.V. +49 (0)30 3087748- 0
Hegelplatz 1 info@ibu-epd.com
10117 Berlin www.ibu-epd.com
Germany
Programme holder
Institut Bauen und Umwelt e.V. +49 (0)30 3087748- 0
Hegelplatz 1 info@ibu-epd.com
10117 Berlin www.ibu-epd.com
Germany
Author of the Life Cycle Assessment
Grundfos Holding A/S +45 87501400
Poul Due Jensens Vej 7 atomic@grundfos.com
8850 Bjerringbro www.grundfos.com
Denmark
Owner of the Declaration
Grundfos Holding A/S +45 87501400
Poul Due Jensens Vej 7 atomic@grundfos.com
8850 Bjerringbro www.grundfos.com
Denmark
12 Environmental-Product Declaration - Grundfos Holding A/S - UPM3 (Composite)
