ENVIRONMENTAL PRODUCT DECLARATION
as per ISO 14025 and EN 15804+A2
Owner of the Declaration Zürcher Ziegeleien AG
Programme holder Institut Bauen und Umwelt e.V. (IBU)
Publisher Institut Bauen und Umwelt e.V. (IBU)
Declaration number EPD-ZZW-20200283-CBB1-EN
Issue date 12.03.2021
Valid to 11.03.2026
Urban cladding tile
Zürcher Ziegeleien AG
www.ibu-epd.com | https://epd-online.com
Umwelt Produktdeklaration Name des Herstellers – Name des Produkts
General Information
ZZ Wancor AG Urban cladding tiles
Programme holder Owner of the declaration
IBU – Institut Bauen und Umwelt e.V. Zürcher Ziegeleien AG
Panoramastr. 1 Eichwatt 1
10178 Berlin CH-8105 Regensdorf
Germany
Declaration number Declared product / declared unit
EPD-ZZW-20200283-CBB1-EN Urban cladding tiles
This declaration is based on the product Scope:
category rules: This EPD covers the Urban ceramic cladding tiles
Ceramic panelling, 07.2014 series produced at one production site in Switzerland
(PCR checked and approved by the SVR) by the company Zürcher Ziegeleien AG. The EPD
document itself refers to the L-Type of the series. In a
public annexe to the EPD, the specific LCA results for
Issue date
the U-Type and T-Type variation are declared as well.
12.03.2021
In the same annexe, representative scenarios for
different sub-construction alternatives (aluminium or
Valid to wood -based) are provided, to allow for a full system
11.03.2026 analysis.
The owner of the declaration shall be liable for the
underlying information and evidence; the IBU shall not
be liable with respect to manufacturer information, life
cycle assessment data and evidences.
The EPD was created according to the specifications
of EN 15804+A2. In the following, the standard will be
simplified as EN 15804.
Verification
The standard EN 15804 serves as the core PCR
Independent verification of the declaration and data
according to ISO 14025:2010
Dipl. Ing. Hans Peters internally x externally
(chairman of Institut Bauen und Umwelt e.V.)
Dr. Alexander Röder Angela Schindler
(Managing Director Institut Bauen und Umwelt e.V.)) (Independent verifier)
Product
Information about the enterprise panels can be installed on common support battens
ZZ Wancor is the Swiss supplier for ceramic building made of wood.
materials. With its two roof tile plants and one brick For the placing on the market of the product in the
plant, it is able to supply its customers with local clay European Union/European Free Trade Association
materials with correspondingly short delivery (EU/EFTA) (with the exception of
distances. Switzerland) Regulation (EU) No. 305/2011 (CPR)
applies. The product needs a declaration of
Product description/Product definition performance taking into consideration EN 1304:2013,
The declared product involves small-format ceramic Clay roofing tiles and fittings and the CE-marking.
cladding tiles made of clay. The panels are For the application and use the respective national
manufactured from various clay masses and differ in provisions apply. Additionally, an European Technical
their surfaces and colours by using different technics in Assessment ETA no. ETA-20/0139 exists for Urban
applying the engobe and different technics of T’s substructure ‘GFT 111’.
roughening the surface. They are single-shell panels
for ventilated façades. The manufacturing corresponds Application
to the extrusion process. Three different types (Urban The systems are attached to a primary substructure.
U, Urban L, Urban T) are produced which differ both in Urban U- and L-Type is fixed by means of a wooden
terms of aesthetics and fastening. The Urban T-type support system, and Urban T-type by means of a
façade panels are connected to the primary façade system-bound aluminium support system. The weights
support system using a system-bound aluminium and number per square metre vary slightly between
substructure. The Urban U and Urban L-type façade the types.
2 Environmental Product Declaration Zürcher Ziegeleien AG – Urban cladding tile
Illustration of a System with Urban U (L) Water absorbtion 0.7 %
Break load NR kN/m
Thermal conductivity NR W/(mK)
Sound absorption coefficient (if
NR %
relevant)
NR = not relevant
Product according to the CPR, based on a hEN:
 Performance data of the product in
accordance with the declaration of
performance with respect to its essential
characteristics according to EN 1304:2013,
Clay roofing tiles and fittings.
 Additionally, for Urban T’s substructure ‘GFT
111’ exist an ETA no. ETA-20/0139.
Illustration of a System with Urban T
Base materials/Ancillary materials
The Urban façade system consists of ceramic
cladding tiles and either a wooden or an aluminum
substructure. The cladding tiles comprise ~95% of clay
(weathered products of feldspathic stones), ~4% of
coloured pigments (metallic oxides for pigmentation of
the raw material), 0.35% of barium carbonate
(mineral), and <1% of surface colour coating (engobes.
The main part of clay is originally from the site of
Laufen and the regional facility surrounding. A quantity
proportion of approximately 12% originates from
Schwarzwald in Germany. Coloured pigments and
surface coatings are additionally purchased from
renowned. Manufacturers of those materials.
This product contains substances listed in the
candidate list (21.06.2013) exceeding 0.1 percentage
by mass: yes.
Technical Data 0.35% of barium sulfate (CAS no.: 7727-43-7)
General Technical Data (U, L, T)
No other REACH-relevant substances according to the
Length: 185 mm candidate list dated 21 June 2013 are used in
Width: 380 mm production.
Height: 39 mm
Thickness: 19 mm Reference service life
Urban cladding tiles do not change after completion of
Further technical details are listed in the specific data the production process. The expected lifespan
sheets or declaration of performance.The declared according to Bundesinstitut für Bau-, Stadt-, und
weight corresponds to the most used type in 2020. Raumforschung (BBSR) is ≥ 50 years. The tiles are
weatherproof, frost-proof, acid-proof as well as colour-
fast and UV-resistant.
Constructional data Replacing a single or several panels is always
possible.
Name Value Unit
Gross density 1770 kg/m3
Bending strength 5.6 kN
LCA: Calculation rules
Declared Unit Sub-construction (declared in public annex to the
EPD)
Urban facade tiles  Aluminium-EPDM (Ethylene Propylene Diene
 L-Type, declared surface weight 47,74 kg/m² Monomer) sub-construction, declared surface
(in EPD document) weight 9,25 kg/m² (7 kg/m² Aluminium, 2,25
 U-Type, declared surface weight 56,42 kg/m² kg/m² EPDM)
(in public annex to EPD)  Wooden sub-construction incl. stainless steel
 T-Type, declared surface weight 41,65 kg/m² screws, declared surface weight 5,192 kg/m²
(in public annex to EPD) (5,02 kg/m² wood, 0,172 kg/m² screws)
3 Environmental Product Declaration Zürcher Ziegeleien AG – Urban cladding tile
Declared unit
Name Value Unit End of Life stage (C1-C4):
Declared unit (L-Type) 1 m2 Module C1: Manual dismantling (no loads).
Grammage (L-Type) 47.74 kg/m2
Layer thickness 0,019 m Module C2: truck transport to waste processing
(50km). The transport distance can, if necessary, be
adjusted at the building level (e.g. for an actual
transport distance of 100 km: multiply the life cycle
System boundary assessment values by a factor of 2).
Type of the EPD: cradle to gate - with options.
Module C3: average loads for waste processing
The background database used is the one from GaBi (shredding). Material losses cosidered: 3%.
Software.
Credits and loads beyond the system boundaries (D):
Production stage (A1-A3): Scenario D / 1: Material recycling as a component of
Module A1 and A2: Provision of clay via excavator and green roof granulate (substitution of lava granulate).
truck transport to the production site.
Scenario D / 2: Material recycling as backfill material
Module A3: Production loads, in particular supply and (substitution of crushed stone).
useage of fuels and auxillary material and measured
emissions from the burning process. Manufacturing of Comparability
packaging material. Basically, a comparison or an evaluation of EPD data
is only possible if all the data sets to be compared
Construction process stage (A4-A5): were created according to EN 15804 and the building
Module A4: Truck transport to the construction site context, respectively the product-specific
(100km). The transport distance can, if necessary, be characteristics of performance, are taken into account.
adjusted at the building level (e.g. for an actual
transport distance of 200 km: multiply the life cycle
assessment values by a factor of 2).
Module A5: emissions from thermal packaging
treatment (resulting credits in module D). Production of
the substructure (representative life cycle assessment
values for wood and aluminum substructures see the
public annex to the EPD document).
Cuttings were not taken into account, as they depend
heavily on the building context. Cuttings can be
estimated using the declared values for the production
stage (e.g. 5% wastage: multiplication of the life cycle
assessment values for A1-A3 by the factor 0.05).
Electricity consumption for installation (mainly use of
hand machines) was not considered.
4 Environmental Product Declaration Zürcher Ziegeleien AG – Urban cladding tile
.
LCA: Scenarios and additional technical information
Characteristic product properties
Information on biogenic Carbon
Information on describing the biogenic Carbon
Content at factory gate
Name Value Unit
Biogenic Carbon Content in
0 kg C
product
Biogenic Carbon Content in
0.743 kg C
accompanying packaging
Transport to the building site (A4)
Name Value Unit
Litres of fuel 0.0993 l/100km
Transport distance 100 km
Capacity utilisation (including
61 %
empty runs)
Reference service life
Name Value Unit
Life Span (according to BBSR) ≥50 a
End of life (C1-C4)
Name Value Unit
Collected separately waste type 47.74 kg
Collected as mixed construction
0 kg
waste
Reuse 0 kg
Recycling 46.3 kg
Energy recovery 0 kg
Landfilling 1.44 kg
5 Environmental Product Declaration Zürcher Ziegeleien AG – Urban cladding tile
LCA: Results
The LCA results for other product variations and the sub-construction can be found in a public annex to this EPD.
To assess specific configurations on building level, the results of the LCA may be scaled linear, by using the
quotient of actual mass per unit area divided by declared mass per unit area as scaling factor (e.g. 50 kg/m² /
47,74 kg/m² = 1,0473 = scaling factor to be applied on all indicators in all life cycle stages).
DESCRIPTION OF THE SYSTEM BOUNDARY (X = INCLUDED IN LCA; ND = MODULE OR INDICATOR NOT
DECLARED; MNR = MODULE NOT RELEVANT)
BENEFITS AND
CONSTRUCTI LOADS
PRODUCT STAGE ON PROCESS USE STAGE END OF LIFE STAGE BEYOND THE
STAGE SYSTEM
BOUNDARIES
6 Environmental Product Declaration Zürcher Ziegeleien AG – Urban cladding tile
lairetam
waR
ylppus tropsnarT
gnirutcafunaM
eht
morf
tropsnarT
etis
eht
ot
etag
ylbmessA esU
ecnanetniaM
riapeR
tnemecalpeR tnemhsibrufeR
ygrene
lanoitarepO esu
retaw
lanoitarepO esu
noitcurtsnoc-eD
noitilomed tropsnarT
gnissecorp
etsaW
lasopsiD -esueR -yrevoceR -gnilcyceR laitnetop
A1 A2 A3 A4 A5 B1 B2 B3 B4 B5 B6 B7 C1 C2 C3 C4 D
X X X X X ND ND MNR MNR MNR ND ND X X X ND X
RESULTS OF THE LCA - ENVIRONMENTAL IMPACT according to EN 15804+A2: 1 m² cladding tile "L-
type", 47,74 kg/m²
Core Indicator Unit A1-A3 A4 A5 C1 C2 C3 D/1 D/2
GWP-total [kg CO2-Eq.] 1.36E+1 3.31E-1 2.88E+0 0.00E+0 1.58E-1 1.28E-1 -1.18E+0 -1.11E+0
GWP-fossil [kg CO2-Eq.] 1.68E+1 3.29E-1 2.09E-1 0.00E+0 1.57E-1 1.27E-1 -1.17E+0 -1.10E+0
GWP-biogenic [kg CO2-Eq.] -3.13E+0 0.00E+0 2.67E+0 0.00E+0 0.00E+0 2.43E-4 -2.04E-3 1.07E-3
GWP-luluc [kg CO2-Eq.] 1.06E-2 2.67E-3 3.19E-5 0.00E+0 1.27E-3 4.68E-4 -2.05E-3 -1.18E-3
ODP [kg CFC11-Eq.] 9.18E-14 3.97E-17 3.79E-16 0.00E+0 1.89E-17 5.41E-16 -1.06E-14 -1.15E-14
AP [mol H+-Eq.] 2.71E-2 3.48E-4 4.10E-4 0.00E+0 1.65E-4 1.20E-3 -3.27E-3 -2.10E-3
EP-freshwater [kg PO4-Eq.] 1.96E-5 1.00E-6 5.73E-8 0.00E+0 4.78E-7 3.04E-7 -1.80E-6 -1.72E-6
EP-marine [kg N-Eq.] 8.62E-3 1.04E-4 1.33E-4 0.00E+0 4.93E-5 5.88E-4 -1.31E-3 -6.35E-4
EP-terrestrial [mol N-Eq.] 9.40E-2 1.24E-3 1.93E-3 0.00E+0 5.91E-4 6.47E-3 -1.43E-2 -6.89E-3
POCP [kg NMVOC-Eq.] 2.52E-2 2.83E-4 3.61E-4 0.00E+0 1.35E-4 1.71E-3 -3.78E-3 -1.83E-3
ADPE [kg Sb-Eq.] 8.06E-6 2.37E-8 5.97E-9 0.00E+0 1.13E-8 1.40E-7 -1.77E-7 -1.82E-7
ADPF [MJ] 1.31E+2 4.40E+0 6.47E-1 0.00E+0 2.10E+0 2.39E+0 -1.93E+1 -1.85E+1
[m³ world-Eq
WDP 3.87E-1 2.95E-3 2.97E-1 0.00E+0 1.40E-3 2.14E-2 -1.06E-1 -1.16E-1
deprived]
GWP = Global warming potential; ODP = Depletion potential of the stratospheric ozone layer; AP = Acidification potential of land and water; EP =
Caption Eutrophication potential; POCP = Formation potential of tropospheric ozone photochemical oxidants; ADPE = Abiotic depletion potential for non-
fossil resources; ADPF = Abiotic depletion potential for fossil resources; WDP = Water (user) deprivation potential
RESULTS OF THE LCA - INDICATORS TO DESCRIBE RESOURCE USE according to EN 15804+A2: 1 m²
cladding tile "L-type", 47,74 kg/m²
Indicator Unit A1-A3 A4 A5 C1 C2 C3 D/1 D/2
PERE [MJ] 5.53E+1 2.48E-1 2.69E+1 0.00E+0 1.18E-1 2.01E-1 -3.86E+0 -4.10E+0
PERM [MJ] 2.67E+1 0.00E+0 -2.67E+1 0.00E+0 0.00E+0 0.00E+0 0.00E+0 0.00E+0
PERT [MJ] 8.20E+1 2.48E-1 1.22E-1 0.00E+0 1.18E-1 2.01E-1 -3.86E+0 -4.10E+0
PENRE [MJ] 1.28E+2 4.41E+0 3.54E+0 0.00E+0 2.10E+0 2.39E+0 -1.93E+1 -1.85E+1
PENRM [MJ] 2.89E+0 0.00E+0 -2.89E+0 0.00E+0 0.00E+0 0.00E+0 0.00E+0 0.00E+0
PENRT [MJ] 1.31E+2 4.41E+0 6.47E-1 0.00E+0 2.10E+0 2.39E+0 -1.93E+1 -1.85E+1
SM [kg] 0.00E+0 0.00E+0 0.00E+0 0.00E+0 0.00E+0 0.00E+0 0.00E+0 0.00E+0
RSF [MJ] 0.00E+0 0.00E+0 0.00E+0 0.00E+0 0.00E+0 0.00E+0 0.00E+0 0.00E+0
NRSF [MJ] 0.00E+0 0.00E+0 0.00E+0 0.00E+0 0.00E+0 0.00E+0 0.00E+0 0.00E+0
FW [m³] 3.30E-2 2.87E-4 6.99E-3 0.00E+0 1.36E-4 6.27E-4 -4.48E-3 -4.78E-3
PERE = Use of renewable primary energy excluding renewable primary energy resources used as raw materials; PERM = Use of
renewable primary energy resources used as raw materials; PERT = Total use of renewable primary energy resources; PENRE = Use of
non-renewable primary energy excluding non-renewable primary energy resources used as raw materials; PENRM = Use of non-
Caption
renewable primary energy resources used as raw materials; PENRT = Total use of non-renewable primary energy resources; SM = Use
of secondary material; RSF = Use of renewable secondary fuels; NRSF = Use of non-renewable secondary fuels; FW = Use of net fresh
water
RESULTS OF THE LCA – WASTE CATEGORIES AND OUTPUT FLOWS according to EN 15804+A2:
1 m² cladding tile "L-type", 47,74 kg/m²
Indicator Unit A1-A3 A4 A5 C1 C2 C3 D/1 D/2
HWD [kg] 4.64E-7 2.05E-7 6.27E-10 0.00E+0 9.74E-8 5.05E-8 -1.10E-7 -3.33E-8
NHWD [kg] 2.98E-1 6.73E-4 3.56E-2 0.00E+0 3.21E-4 7.22E-4 -8.24E-3 -1.94E+0
RWD [kg] 2.24E-3 5.45E-6 3.60E-5 0.00E+0 2.60E-6 1.92E-5 -1.28E-3 -1.38E-3
CRU [kg] 0.00E+0 0.00E+0 0.00E+0 0.00E+0 0.00E+0 0.00E+0 0.00E+0 0.00E+0
MFR [kg] 0.00E+0 0.00E+0 0.00E+0 0.00E+0 0.00E+0 4.63E+1 0.00E+0 0.00E+0
MER [kg] 0.00E+0 0.00E+0 0.00E+0 0.00E+0 0.00E+0 0.00E+0 0.00E+0 0.00E+0
EEE [MJ] 0.00E+0 0.00E+0 4.27E+0 0.00E+0 0.00E+0 0.00E+0 0.00E+0 0.00E+0
EET [MJ] 0.00E+0 0.00E+0 7.67E+0 0.00E+0 0.00E+0 0.00E+0 0.00E+0 0.00E+0
HWD = Hazardous waste disposed; NHWD = Non-hazardous waste disposed; RWD = Radioactive waste disposed; CRU = Components
Caption for re-use; MFR = Materials for recycling; MER = Materials for energy recovery; EEE = Exported electrical energy; EEE = Exported
thermal energy
RESULTS OF THE LCA – additional impact categories according to EN 15804+A2-optional:
1 m² cladding tile "L-type", 47,74 kg/m²
Indicator Unit A1-A3 A4 A5 C1 C2 C3 D/1 D/2
[Disease
PM ND ND ND ND ND ND ND ND
Incidence]
[kBq U235-
IR ND ND ND ND ND ND ND ND
Eq.]
ETP-fw [CTUe] ND ND ND ND ND ND ND ND
HTP-c [CTUh] ND ND ND ND ND ND ND ND
HTP-nc [CTUh] ND ND ND ND ND ND ND ND
SQP [-] ND ND ND ND ND ND ND ND
PM = Potential incidence of disease due to PM emissions; IR = Potential Human exposure efficiency relative to U235; ETP-fw = Potential
Caption comparative Toxic Unit for ecosystems; HTP-c = Potential comparative Toxic Unit for humans (cancerogenic); HTP-nc = Potential
comparative Toxic Unit for humans (not cancerogenic); SQP = Potential soil quality index
For the indicator IRP:
This impact category deals mainly with the eventual impact of low dose ionizingradiation on human health of the
nuclear fuel cycle. It does not consider effects due to possiblenuclear accidents, occupational exposure nor due to
radioactive waste disposal in undergroundfacilities. Potential ionizing radiation from the soil, from radon and from
some construction materials is also not measured by this indicator.
For the indicators ADPE, ADPF, WDP, ETP-fw, HTP-c, HTP-nc, SQP:
The results of this environmental impact indicator shall be used with care as the uncertainties on these results are
high or as there is limited experienced with the indicator.
References
Standards European Technical Assessment ETA no. ETA-
20/0139 from 2020/03/13
EN 1304 Technical Assessment Body issuing the ETA and
EN 1304:2005: Clay roofing tiles and fittings - Product designated according to Article 29 of the Regulation
definitions and specifications (EU) No 305/2011: ETA-Danmark A/S
EN 15804+A2 GaBi Software
EN 15804:2019+A2, Sustainability of construction GaBi Software and databases, SP40, Sphera Solution
works — Environmental Product Declarations — Core GmbH, 2020.
rules for the product category of construction products.
IBU 2016
ISO 14025 Institut Bauen und Umwelt e.V.: General Programme
DIN EN ISO 14025:2011-10, Environmental labels and Instructions for the Preparation of EPDs at the Institut
declarations — Type III environmental declarations — Bauen und Umwelt e.V. Version 1., Berlin: Institut
Principles and procedures. Bauen und Umwelt e.V., 2016.
www.ibu-epd.com.
European Chemicals Agency
Substances restricted under REACH
https://echa.europa.eu/de/substances-restricted-under-
reach
Regulation (EU) No 305/2011
Harmonised conditions for the marketing of
construction products and repealing Council Directive
89/106EEC Text with EEA relevance
Public annex:
PCR Product Category Rules for Building-Related
Further References Products and Services
Part A: Calculation Rules for the life Cycle Assessment
BBSR - Bundesinstitut für Bau-, Stadt- und and Requirements on the Project Report according to
Raumforschung EN 15804+A2:2019
Service Life of Building Components; version Part B: Requirements on the EPD for Ceramic
24.02.2017. panelling
https://www.nachhaltigesbauen.de/fileadmin/pdf/Nutzu
ngsdauer_Bauteile/BNB_Nutzungsdauern_von_Bauteil
en_2017-02-24.pdf
7 Environmental Product Declaration Zürcher Ziegeleien AG – Urban cladding tile
Publisher
Institut Bauen und Umwelt e.V. Tel +49 (0)30 3087748- 0
Panoramastr. 1 Fax +49 (0)30 3087748- 29
10178 Berlin Mail info@ibu-epd.com
Germany Web www.ibu-epd.com
Programme holder
Institut Bauen und Umwelt e.V. Tel +49 (0)30 - 3087748- 0
Panoramastr 1 Fax +49 (0)30 – 3087748 - 29
10178 Berlin Mail info@ibu-epd.com
Germany Web www.ibu-epd.com
Author of the Life Cycle
Assessment Tel +49 711 341817-0
Sphera Solutions GmbH Fax +49 711 341817-25
Hauptstraße 111- 113 Mail info@sphera.com
70771 Leinfelden-Echterdingen Web www.sphera.com
Germany
Owner of the Declaration
Zürcher Ziegeleien AG Tel 0041 58 219 09 09
Eichwatt 1 Fax 0041 58 219 09 99
8105 Regensdorf Mail info@zz-ag.ch
Switzerland Web www.zz-ag.ch
