ENVIRONMENTAL PRODUCT DECLARATION
as per ISO 14025 and EN 15804+A2
Owner of the Declaration HALTON FOODSERVICE
Publisher Institut Bauen und Umwelt e.V. (IBU)
Programme holder Institut Bauen und Umwelt e.V. (IBU)
Declaration number EPD-HAL-20240073-IBA1-EN
Issue date 27/08/2024
Valid to 26/08/2029
UVI/F - Capture Ray™ hood
HALTON FOOD SERVICE
www.ibu-epd.com | https://epd-online.com
1. General Information
HALTON FOOD SERVICE UVI/F - Capture Ray™ hood
Programme holder Owner of the declaration
IBU – Institut Bauen und Umwelt e.V. HALTON FOODSERVICE
Hegelplatz 1 Zone Technoparc Futura CS 80102
10117 Berlin 62402 BETHUNE Cedex
Germany France
Declaration number Declared product / declared unit
EPD-HAL-20240073-IBA1-EN 1 linear metre of UVI/F hood, used to extract heat and cooking steam for
365 days a year, for 8 hours a day, for 15 years
This declaration is based on the product category rules: Scope:
Ventilation systems for commercial kitchens, 24/01/2024 This document refers to UVI/F hood produced by HALTON
(PCR checked and approved by the SVR) FOODSERVICE in France.
This EPD represents the declaration of a specific product UVI/F Hood, with
the declared unit of 1 linear metre of hood, used to extract heat and
Issue date cooking steam for 365 days a year, for 8 hours a day, for 15 years.
The data collection for the ecological assessment occurred plant specific
27/08/2024
with current annual data. Consequently, the Life Cycle Assessment is
representative for this product.
The owner of the declaration shall be liable for the underlying information
Valid to
and evidence; the IBU shall not be liable with respect to manufacturer
26/08/2029 information, life cycle assessment data and evidences.
The EPD was created according to the specifications of EN 15804+A2. In
the following, the standard will be simplified as EN 15804.
Verification
The standard EN 15804 serves as the core PCR
Independent verification of the declaration and data according to ISO
14025:2011
internally X externally
Dipl.-Ing. Hans Peters
(Chairman of Institut Bauen und Umwelt e.V.)
Florian Pronold Dr. Matthew Fishwick,
(Managing Director Institut Bauen und Umwelt e.V.) (Independent verifier)
1 Environmental Product Declaration - HALTON FOOD SERVICE - UVI/F - Capture Ray™ hood
2. Product
Biocide products were added to this construction product or it
2.1 Product description/Product definition has been treated with biocide products (this then concerns a
The UVI/F reduces the grease build up in the ductwork to a treated product as defined by the (EU) Ordinance on Biocide
negligible level. Capture Ray™ technology is based on the use Products No. 528/2012): no.
of UV-C lamps. The Neutralization of grease particles and
vapors as well as the mitigation of the cooking odors depend on 2.6 Manufacture
two simultaneous reactions. Photolysis is the direct effect of Manufacturing and packaging of the UVI/F hood at the
UV-C radiation. It works by photodecomposition whereby production site. In this case, manufacturing mainly refers to the
grease molecules are broken down by photons. Ozonolysis is assembling, configuring, and testing of the hoods from pre-
the oxidation of grease molecules by ozone that is generated made parts. The assessment covers the electricity, LPG
by the lamps. As ozone is a gas, it is carried with the airflow. consumption for forklifts and water use needed during the
Oxidation therefore takes place in the hoods and ventilated production process. The electricity is modelled as site-specific
ceilings' exhaust plenum as well as in the ductwork. The energy mixes provided by local energy companies.The waste
product is manufactured from steel, electronics, aluminium, streams from the manufacturing site include, wastewater, wood
plastic. waste, cardboard, plastic and metal scrap (stainless steel and
galvanised steel sheets).
The Capture Jet™ technology (KVI/F) is related to the Any production waste generated is disposed of according by
association of two sets of nozzles supplied with an extremely Halton's waste contractor.
low supply air volume (a maximum of 30 m³/h/m of hood).
These nozzles fit to the lower part of the hood front as well as 2.7 Environment and health during manufacturing
the sides, encircling the perimeter of the covered cooking Workplace and emission limits are regularly monitored and are
areas. The horizontal nozzles increase the push/pull of the far below the prescribed limits.
thermal plume and smoke from the lower part of the hood front
2.8 Product processing/Installation
due to the Venturi effect. It provides an assist to push vapours
back towards the filters. For the placing on the market of the The hood is installed in about 10 hours by 2 employees. The
product in the European Union/European Free Trade hood is fixed by hand to the ceiling with the help of a lifter and
Association (EU/EFTA) (with the exception of Switzerland) some fixation devices.
Regulation (EU) No. 305/2011 (CPR) applies. The product
2.9 Packaging
needs a declaration of performance taking into consideration
For product protection the hoods are individually packed in a
EN and the CE-marking.
cardboard box. All packaged products are wrapped with (low
For the application and use the respective national provisions
density polyethylene) PEBD/LDPE film on a wood pallet.
apply.
2.10 Condition of use
2.2 Application
To ensure the longevity of the product, a weekly cleaning (using
The UVI/F hood is used for professional kitchens. They can be
water with 1.5% soap) and annual check-up on different hood
installed above the cooking appliances and is used to remove
parameters (Capture jets state, lighting state, filters (state and
fumes, odors, heat, humidity, and any airborne grease from the
number), k factor, exhaust rates in intake rates) are
environment.
recommended.
2.3 Technical Data
2.11 Environment and health during use
The technical properties are project-dependent (Airflow range).
The products do not emit any contaminants or substances that
The dimensions of the reference product is specified in the
are harmful to the environment or health during the use phase.
table below.
2.12 Reference service life
The service life is validated if the hood is installed following the
Constructional Data installation procedure. Reference service life for the cooker
Name Value Unit hoods is assumed 15 years.
The reference service life is based on the empirical value for
Length 1000 mm
the hoods when used in accordance with the care instructions.
Width 1400 mm
Height 500 mm 2.13 Extraordinary effects
Weight 120 kg Fire
power consumption (operation) 457 W The products are not classified as building materials (building
products) and are not subject to DIN 4102 and EN 13501-1.
Performance data of the product with respect to its Water
characteristics in accordance with the relevant technical No water-hazardous, toxic substances are washed-out to the
provision (no CE-marking). environment and water.
2.4 Delivery status
Mechanical destruction
The products vary in size as they are not catalogue products.
There are no relevant environmental impacts associated with
mechanical destruction.
2.5 Base materials/Ancillary materials
This product/article/at least one partial article contains other 2.14 Re-use phase
Carcinogenic, mutagenic, reprotoxic (CMR) substances in
The UVI/F are not taken back by the manufacturer for the
categories 1A or 1B which are not on the candidate list,
purpose of reuse. Users can disassemble the products
exceeding 0.1 percentage by mass: no.
repeatedly within the reference utilization period and reuse it
elsewhere.
2 Environmental Product Declaration - HALTON FOOD SERVICE - UVI/F - Capture Ray™ hood
2.15 Disposal 2.16 Further information
Disassembly of the products consists of the same steps as Additional information about our products can be found on
assembly, in reverse order. The product falls under the Waste Halton-website: www.halton.com.
from Electrical and Electronic Equipment (WEEE).
3. LCA: Calculation rules
The hoods haven't significant impact for emission in indoor air
3.1 Declared Unit or in water during use.
The declared unit is: '1 linear metre of hood, used to extract
heat and cooking steam for 365 days a year, for 8 hours a day, Module B2:
for 15 years'.' - a weekly cleaning with 5L of water containing 1,5% soap.
Declared unit - annual check-up by a technician on different hood parameters
(Capture jets state, lighting state, filters (state and number), k
Name Value Unit
factor, exhaust rates in intake rates) modelled with
Declared unit 1 rm
transportation of one technician in light commercial vehicle (100
Mass per Unit 120 kg km).
linear density 120 kg/rm - 2 UV light replacements during the reference life service.
- End-of-life treatment of 2 UV light tubes during SLR with
Other declared units are allowed if the conversion is shown
transportation included
transparently.
Module B6 et B7
3.2 System boundary The hood is designed for heavy duty industrial usage. To reflect
the most average scenario the hood will be functioning 8 hours
This representative EPD follows the EPD type "cradle to grave".
a days 7 days a week. Electricity (B6) is required to use the
The following life cycle modules are declared:
products.
Modules A1-A3
The product stage begins with considering the production of the
Modules C1-C4
necessary raw materials (metals, electronics, packaging
The module includes the environmental impacts for dismantling
materials), including all corresponding upstream chains and the
of the products and the treatment of the UVI/F hood waste until
actual procurement transports.
the end-of-waste status (EoW) is reached, including the
Furthermore, the entire manufacturing phase was mapped,
associated transports at the end of the product life cycle.
including the treatment of production waste until the end-of
The product is assumed to be removed manually at the same
waste status (EoW) was reached.
time as the building is demolished. No scenario has been
developed for stage C1.
Module A4
The transport model considers a construction site in Europe.
The hood and the ceiling beam are removed separately.
The scenario for the distribution stage considers a average
Dismantling of product components at recycling facility. Based
distance to serve the entire European area from the Halton's
on the material, components are either recycled, incinerated, or
plant. The quantity transported corresponds to the transport of
landfilled depending on the material.
products and their packaging to the construction site.
Stage C3 represents the impact of a conventional scrap
Module A5
processing site, with sorting, shearing, shredding, separation.
The hood is delivered at the right size on the installation site. It
is installed in about 10 hours by 2 employees. The hood is fixed
Module D
to the ceiling with the help of a lifter and some fixation devices.
Identification of the benefits and costs of the product outside
the system boundary.
Complementary products for installation include a ceiling beam
Recycling of metal scrap results in credits of the respective raw
in galvanised steel. This additional product is supplied by
materials for the primary material portion of the input. The loads
Halton. Their production and packaging are considered in A1,
of the waste incineration and recycling processes are assigned
their transport in A3 and A4 and the end-of-life of their
to the respective modules (A3, A5 and C3) and not to module
packaging in A5.
D.
Others complementary products are used to fix the MUPRO
3.3 Estimates and assumptions
Ceiling beam (clip, pin, screw). They must be purchased by the
Energy and water consumption during production could only be
installer because they depend on ceiling type (metallic,
determined on existing products and not on the average
concrete or wood). They are not considered in this study.
product.
The application phase considers: 3.4 Cut-off criteria
- Transportation of material lifter to installation site : 2500 kg on
Cut-off criteria follow EN15804 and PCR Part A. No flows have
30 km.
been deliberately omitted from the system boundaries.
- Waste treatment (product packaging) :
3.5 Background data
All background data was considered using data from the
Modules B1 & B3-B5 & B7 Ecoinvent 3.7.1 database or literary sources.
These modules were considered but evaluated as not relevant
for the products and considered as zero. Products do not 3.6 Data quality
require repair (B3)/replacement (B4)/rehabilitation (B5). Site-specific production data has been collected for 2021 from
the production site. The upstream and downstream processes
3 Environmental Product Declaration - HALTON FOOD SERVICE - UVI/F - Capture Ray™ hood
have been modelled based on environmental data from generic consumption of electricity and water in Halton's plant were
databases ecoinvent. The collected data was reviewed in terms allocated per working hours for assembly of each product. No
of consistency, and it is estimated as good quality. other allocations were made in this assessment. The cut-off
end-of-life allocation approach was used throughout.
3.7 Period under review
The data is therefore based on 2021. All information is based 3.10 Comparability
on averaged data for 12 consecutive months. Basically, a comparison or an evaluation of EPD data is only
possible if all the data sets to be compared were created
3.8 Geographic Representativeness according to EN 15804 and the building context, respectively
Land or region, in which the declared product system is the product-specific characteristics of performance, are taken
manufactured, used or handled at the end of the product´s into account. According to the EN 15804 standard,
lifespan: Europe environmental declarations for construction products may not
be comparable if they have not been prepared in accordance
with that standard or if a different notified unit has been
3.9 Allocation
used.The LCA was conducted using SimaPro 9.2.0.2. software.
Allocation has been avoided whenever possible by collecting
All background data was considered using data from the
product specific environmental data. In case of manufacturing
ecoinvent 3.7.1 (cut-off) database or literary sources.
energy use, where allocation could not be avoided, the
4. LCA: Scenarios and additional technical information
without energy recovery, 38% landfill.
Characteristic product properties of biogenic carbon
The biogenic carbon content quantifies the amount of biogenic Service Life
carbon in a construction product leaving the factory gate, and it HALTON declares a Service Life of 15 years as an empirical
shall be separately declared for the product and for any value for the hoods when used in accordance with the care
accompanying packaging. instructions.
Maintenance (B2)
The mass of packaging containing biogenic carbon is declared.
Name Value Unit
Note: 1 kg of biogenic carbon is equivalent to 44/12 kg of CO . Total number of check-up
2 60
during SRL
Name Value Unit
Estimated distance for round
Biogenic carbon content of the product 0 kg.C 100 km
trip
Biogenic carbon content of associated packaging 15.2 kg.C
Estimated weight of
technician doing the check 80 kg
The scenarios and assumptions applied in this study for all the up.
life cycle stages included are based on data provided by Halton
2 replacements of UV light 5.40E-
and correspond to the most likely scenario. The following kg
during SLR 01
scenarios and general assumptions were made in the studied
3.09E m3 of water containing
lifecycle stages: Weekly cleaning
+03 1,5% soap /DVR
Transport to the building site (A4) Operational energy use (B6-B7)
Name Value Unit Name Value Unit
Transport of distance 1631.4 km Energy demand 1334 kWh/year
Capacity utilization (including empty runs) ~19 %
End of life (C1-C4)
Installation into the building (A5) Name Value Unit
Name Value Unit Transport to treatment site 50 km
Material loss 0 % The following end of life scenarios are considered for the
The following end of life scenarios are considered for product:
packaging:
NHW Plastic : 1.27E+00 kg → 41% recycling, 37% incineration
NHW Plastic : 1.43E+00 kg → 41% recycling, 37% incineration without energy recovery, 22% landfill
without energy recovery, 22% landfill. NHW Steel : 1.12E+02 kg → 90% recycling, 10% landfill
NHW Glass : 6.97E-01 kg → 100% landfill
NHW Cardboard : 4.33E+00 kg → 82% recycling, 9% NHW WEE : 8.79E+00 kg → 74,7% recycling, 1.8% reuse,
incineration without energy recovery, 9% landfill. 9.7% incineration without energy recovery, 13.8% landfill.
NHW Wood : 3.00E+01 kg → 31% recycling, 31% incineration
4 Environmental Product Declaration - HALTON FOOD SERVICE - UVI/F - Capture Ray™ hood
5. LCA: Results
The following table shows the result of the LCA for 1 m of a UVI/F hood.
DESCRIPTION OF THE SYSTEM BOUNDARY (X = INCLUDED IN LCA; MND = MODULE OR INDICATOR NOT DECLARED; MNR
= MODULE NOT RELEVANT)
Benefits and
Construction loads beyond
Product stage Use stage End of life stage
process stage the system
boundaries
la ire ta m w a Ry lp p u s tro p s n a rT g n iru tc a fu n a M e h t m o rf tro p s n a rTe tis e h t o t e ta g y lb m e s s A e s U e c n a n e tn ia M ria p e R tn e m e c a lp e R tn e m h s ib ru fe R y g re n e la n o ita re p Oe s u re ta w la n o ita re p Oe s u n o itc u rts n o c -e Dn o itilo m e d tro p s n a rT g n is s e c o rp e ts a W la s o p s iD -e s u e R-y re v o c e R-g n ilc y c e Rla itn e to p
A1 A2 A3 A4 A5 B1 B2 B3 B4 B5 B6 B7 C1 C2 C3 C4 D
X X X X X MND X MNR MNR MNR X MND X X X X X
RESULTS OF THE LCA - ENVIRONMENTAL IMPACT according to EN 15804+A2: 1 m UVIF Hood
Parameter Unit A1-A3 A4 A5 B2 B6 C1 C2 C3 C4 D
GWP-total kg CO 2 eq 4.33E+03 3.26E+01 1.14E+02 1.44E+03 8.39E+03 0 9.95E-01 2.62E+00 4.15E+00 -1.72E+02
GWP-fossil kg CO 2 eq 4.36E+03 3.26E+01 4.6E+01 1.27E+03 8.32E+03 0 9.95E-01 6.79E-01 3.6E+00 -1.72E+02
GWP-
biogenic kg CO 2 eq -3.56E+01 1.26E-02 6.8E+01 2.1E+01 4.8E+01 0 3.83E-04 1.94E+00 5.48E-01 -3.35E-01
GWP-luluc kg CO 2 eq 6.74E+00 1.12E-02 2.17E-02 1.45E+02 1.73E+01 0 3.41E-04 6.03E-04 7.33E-05 -7.18E-02
ODP kg CFC11 eq 3.17E-04 7.41E-06 8.64E-06 2.09E-04 4.22E-04 0 2.26E-07 1.35E-07 4.81E-08 -6.75E-06
AP mol H+ eq 2.67E+01 9.07E-02 1.55E-01 7.41E+00 4.54E+01 0 2.77E-03 7.26E-03 1.76E-03 -6.24E-01
EP-
kg P eq 6.72E-01 2.44E-04 4.88E-04 7.82E-01 8.82E-01 0 7.45E-06 6.35E-05 8.53E-06 -8.54E-03
freshwater
EP-marine kg N eq 5.3E+00 1.85E-02 5.78E-02 3.03E+00 6.06E+00 0 5.63E-04 4.04E-03 1.26E-03 -1.47E-01
EP-terrestrial mol N eq 6.04E+01 2.05E-01 4.75E-01 2.4E+01 6.97E+01 0 6.26E-03 2.72E-02 7.48E-03 -1.58E+00
kg NMVOC
POCP 1.59E+01 7.86E-02 1.51E-01 6.91E+00 1.9E+01 0 2.4E-03 6.59E-03 2.18E-03 -7.82E-01
eq
ADPE kg Sb eq 1.25E+00 1.2E-04 2.61E-04 2.5E-02 7.57E-02 0 3.66E-06 6.69E-05 6.27E-07 -2.42E-04
ADPF MJ 5.57E+04 4.95E+02 6.03E+02 1.79E+04 1.76E+05 0 1.51E+01 6.42E+00 2.87E+00 -1.7E+03
m3 world eq
WDP 1.1E+03 1.43E+00 2.29E+00 7.67E+02 1.8E+03 0 4.36E-02 -1.29E-01 1.94E-01 1.3E+00
deprived
GWP = Global warming potential; ODP = Depletion potential of the stratospheric ozone layer; AP = Acidification potential of land and water; EP =
Eutrophication potential; POCP = Formation potential of tropospheric ozone photochemical oxidants; ADPE = Abiotic depletion potential for non-fossil
resources; ADPF = Abiotic depletion potential for fossil resources; WDP = Water (user) deprivation potential)
RESULTS OF THE LCA - INDICATORS TO DESCRIBE RESOURCE USE according to EN 15804+A2: 1 m UVIF Hood
Parameter Unit A1-A3 A4 A5 B2 B6 C1 C2 C3 C4 D
PERE MJ 7.22E+03 6.76E+00 1.26E+01 2.13E+03 3.17E+04 0 2.06E-01 1.86E+00 7.49E-02 -2.38E+02
PERM MJ 5.66E+02 0 -2.15E+02 0 0 0 0 0 0 0
PERT MJ 7.78E+03 6.76E+00 -2.03E+02 2.13E+03 3.17E+04 0 2.06E-01 1.86E+00 7.49E-02 -2.38E+02
PENRE MJ 5.55E+04 4.95E+02 6.28E+02 1.81E+04 1.73E+05 0 1.51E+01 6.31E+00 2.87E+00 -1.69E+03
PENRM MJ 1.12E+02 0 -2.52E+01 0 0 0 0 0 -4.79E+00 0
PENRT MJ 5.56E+04 4.95E+02 6.02E+02 1.8E+04 1.73E+05 0 1.51E+01 6.3E+00 -1.92E+00 -1.69E+03
SM kg 0 0 0 0 0 0 0 0 0 0
RSF MJ 0 0 0 0 0 0 0 0 0 0
NRSF MJ 0 0 0 0 0 0 0 0 0 0
FW m3 6.51E+01 6.76E-02 1.19E-01 2.64E+01 1.45E+02 0 2.06E-03 1.97E-03 5.56E-03 -1.33E-01
PERE = Use of renewable primary energy excluding renewable primary energy resources used as raw materials; PERM = Use of renewable primary
energy resources used as raw materials; PERT = Total use of renewable primary energy resources; PENRE = Use of non-renewable primary energy
excluding non-renewable primary energy resources used as raw materials; PENRM = Use of non-renewable primary energy resources used as raw
materials; PENRT = Total use of non-renewable primary energy resources; SM = Use of secondary material; RSF = Use of renewable secondary fuels;
NRSF = Use of non-renewable secondary fuels; FW = Use of net fresh water
RESULTS OF THE LCA – WASTE CATEGORIES AND OUTPUT FLOWS according to EN 15804+A2:
1 m UVIF Hood
Parameter Unit A1-A3 A4 A5 B2 B6 C1 C2 C3 C4 D
HWD kg 7.83E+02 3.4E-01 3.31E+00 7.39E+01 1.94E+02 0 1.04E-02 5.39E-01 2.24E-01 -1.72E+01
NHWD kg 6.1E+03 2.81E+01 3.8E+01 9.98E+02 3.18E+03 0 8.59E-01 2.38E+00 1.15E+01 -4.05E+02
RWD kg 1.77E-01 3.38E-03 4.02E-03 1.03E-01 1.24E+00 0 1.03E-04 1.01E-04 1.58E-05 -2.89E-03
CRU kg 0 0 0 7.39E+01 1.94E+02 0 0 5.39E-01 0 -1.72E+01
MFR kg 4.05E+01 0 1.34E+01 9.98E+02 3.18E+03 0 0 2.38E+00 0 -4.05E+02
MER kg 0 0 0 1.03E-01 1.24E+00 0 0 1.01E-04 0 -2.89E-03
EEE MJ 0 0 0 0 0 0 0 1.58E-01 0 0
5 Environmental Product Declaration - HALTON FOOD SERVICE - UVI/F - Capture Ray™ hood
EET MJ 0 0 0 0 0 0 0 0 0 0
HWD = Hazardous waste disposed; NHWD = Non-hazardous waste disposed; RWD = Radioactive waste disposed; CRU = Components for re-use;
MFR = Materials for recycling; MER = Materials for energy recovery; EEE = Exported electrical energy; EET = Exported thermal energy
RESULTS OF THE LCA – additional impact categories according to EN 15804+A2-optional:
1 m UVIF Hood
Parameter Unit A1-A3 A4 A5 B2 B6 C1 C2 C3 C4 D
Disease
PM 2.31E-04 2.05E-06 2.11E-06 1.19E-04 1.2E-04 0 6.27E-08 1.13E-07 3.4E-08 -1.08E-05
incidence
IR kBq U235 eq 2.27E+02 2.17E+00 2.66E+00 7.82E+01 1.52E+03 0 6.63E-02 9.28E-02 1.07E-02 -2.64E+00
ETP-fw CTUe 3.21E+05 3.8E+02 5.97E+02 3.55E+04 1.1E+05 0 1.16E+01 2.79E+02 8.11E+01 -4.08E+03
HTP-c CTUh 1.53E-05 1.35E-08 2.54E-08 1.97E-06 3.27E-06 0 4.11E-10 1.98E-09 1.29E-09 -1.04E-06
HTP-nc CTUh 1.34E-04 3.71E-07 5.5E-07 2.23E-05 8.64E-05 0 1.13E-08 4.37E-08 1.54E-08 -3.59E-06
SQP SQP 4.73E+04 5.06E+02 4.24E+02 3.12E+04 5.65E+04 0 1.54E+01 1.08E+02 4.55E+00 -2.34E+03
PM = Potential incidence of disease due to PM emissions; IR = Potential Human exposure efficiency relative to U235; ETP-fw = Potential comparative
Toxic Unit for ecosystems; HTP-c = Potential comparative Toxic Unit for humans (cancerogenic); HTP-nc = Potential comparative Toxic Unit for humans
(not cancerogenic); SQP = Potential soil quality index
Disclaimer 1 – for the indicator “Potential Human exposure efficiency relative to U235”. This impact category deals mainly with the
eventual impact of low-dose ionizing radiation on human health of the nuclear fuel cycle. It does not consider effects due to possible
nuclear accidents, occupational exposure or radioactive waste disposal in underground facilities. Potential ionizing radiation from the
soil, radon and from some construction materials is also not measured by this indicator.
Disclaimer 2 – for the indicators “abiotic depletion potential for non-fossil resources”, “abiotic depletion potential for fossil resources”,
“water (user) deprivation potential, deprivation-weighted water consumption”, “potential comparative toxic unit for ecosystems”,
“potential comparative toxic unit for humans – cancerogenic”, “Potential comparative toxic unit for humans - not cancerogenic”,
“potential soil quality index”. The results of this environmental impact indicator shall be used with care as the uncertainties on these
results are high as there is limited experience with the indicator.
6. LCA: Interpretation
The dominance analysis shows that modules B6 and A1 are the
dominant life cycle stages in most of the categories. B6
dominates most indicators due the energy demand in electricity
for using. The modules A1-A3 have great contributions to all
categories especially for the Depletion of abiotic resources -
minerals and metals. In this indicator the provision of
electronics component has the largest contribution. The end-of-
life stage has no significant influence on the environmental
indicators. The environmental burdens from the transports
(modules A4 and C2) account less than 1% of the total burdens
from the transports in all cases.
7. Requisite evidence
8. References
PCR 2020, Part A EN 15804:2012+A2:2019+AC:2021, Sustainability of
Institut Bauen und Umwelt e.V., Berlin (pub.): Product construction works — Environmental Prouct Declarations —
Category Rule for Construction Products from the Core rules for the product category of construction products.
range of Environmental Product Declarations of
Institute Bauen und Umwelt (IBU), Part A: Calculation ISO 14025
rules for the Life Cycle Assessment and requirements EN ISO 14025:2011, Environmental labels and declarations —
on the project report according to EN 15804+A2. Type III environmental declarations — Principles and
Version 2020-07. procedures.
www.ibu-epd.com
DIN 4102-1
PCR 2024, Part B DIN 4102-1: Fire behaviour of building materials and building
Product Category Rules for Construction Products, components - Part 1: Building materials; concepts,
Part B: Ventilations systems for commercial kitchens, requirements and tests. 1998-05
24/01/2024
DIN EN 13501-1
EN 15804 DIN EN 13501-1:2019-05: Fire classification of construction
6 Environmental Product Declaration - HALTON FOOD SERVICE - UVI/F - Capture Ray™ hood
products and building elements - Part 1: Classification using 93/105/EC and 2000/21/EC, 2006-12.
data from reaction to fire tests; German version EN 13501-
1:2018 Biocide Guideline
Regulation (EU) No. 528/2012 of the European
/Further References Parliament and of the Council of 22 May 2012
concerning the making available on the market and
SimaPro 9.2.0.2 use of biocidal products
CPR
WEEE Directive (EU) No. 305/2011 of the European
Waste Electrical and Electronic Equipment Directive : Act Parliament and Council dated 9 March 2011
governing the requirements on utilisation and disposal of establishing harmonised conditions for marketing
WEEE. construction products and replacing Council Guideline
89/106/EEC
REACH Regulation Ecoinvent
Regulation (EC) No. 1907/2006 of the European Parliament Ecoinvent database version 3.7.1
and of the Council of 18 December 2006
concerning the Registration, Evaluation, Authorisation
and Restriction of Chemicals (REACH), establishing a IBU 2021
European Chemicals Agency, amending Directive Institut Bauen und Umwelt e.V.: General Instructions for the
1999/45/EC and repealing Council Regulation (EEC) EPD programme of Institut Bauen und Umwelt e.V., Version
No. 793/93, Commission Regulation (EC) No. 1488/94 2.0, Berlin: Institut Bauen und Umwelt e.V., 2021
as well as Council Directive 76/769/EEC and www.ibu-epd.com
Commission Directives 91/155/EEC, 93/67/EEC,
7 Environmental Product Declaration - HALTON FOOD SERVICE - UVI/F - Capture Ray™ hood
Publisher
Institut Bauen und Umwelt e.V. +49 (0)30 3087748- 0
Hegelplatz 1 info@ibu-epd.com
10117 Berlin www.ibu-epd.com
Germany
Programme holder
Institut Bauen und Umwelt e.V. +49 (0)30 3087748- 0
Hegelplatz 1 info@ibu-epd.com
10117 Berlin www.ibu-epd.com
Germany
Author of the Life Cycle Assessment
CSTB 04 56 14 72 62
rue Joseph Fourier 24 cecile.magnin-feysot@cstb.fr
38400 Saint-Martin-d'Hères https://www.cstb.fr/fr/
France
Owner of the Declaration
HALTON FOODSERVICE 06.14.71.06.55
Zone Technoparc Futura CS 80102 arnaud.kazmierczak@halton.com
62402 BETHUNE Cedex https://www.halton.com/fr/
France
8 Environmental Product Declaration - HALTON FOOD SERVICE - UVI/F - Capture Ray™ hood
