—
EPD
Environmental Product Declaration
Vacuum Interrupter VG4-S
Production site: Ratingen, Germany
DOCUMENT KIND IN COMPLIANCE WITH
Environmental Product Declaration ISO 14025 and EN50693
PROGRAM OPERATOR PUBLISHER
The Norwegian EPD Foundation The Norwegian EPD Foundation
REGISTRATION NUMBER OF THE PROGRAM OPERATOR ISSUE DATE
NEPD-3887-2831-EN 11.11.2022
VALID TO STATUS SECURITY LEVEL
Approved Public
2027-11-11
OWNING ORGANIZATION DECLARATION NUMBER REV. LANG. PAGE
ABB Switzerland Ltd 3XAA008728 B001 EN 1/19
© Copyright 2022 ABB. All rights reserved.
ver2-120423
ENVIRONMENTAL PRODUCT DECLARATION
EPD Owner ABB Switzerland Ltd, Group Technology Management
Manufacturer name and ABB AG
address Oberhausener Str. 33, 40472 Ratingen
Organization no CH-020.3.900.058-8
Seila Rodriguez Vilches – seila.rodriguez-vilches@ch.abb.com
Company contact
Sustainability Product Manager
The Norwegian EPD Foundation
Post Box 5250 Majorstuen, 0303 Oslo, Norway
Program operator
Ph.:+47 23 08 80 00
email: post@epd-norge.no
VG4-S
FU: The functional unit of this study is to establish or
interrupt the electrical continuity of a circuit within a
Declared product,
switchgear compartment in power systems during a
functional unit (FU) and
reference service life of 20 years including related accessories
reference flow (RF)
and packaging.
RF: A single vacuum interrupter including related accessories
and packaging.
Vacuum interrupters (VIs) are the core component for all
switching applications in medium voltage. The main purpose
of the vacuum interrupter is to establish or to interrupt a
Product description
current flow by separation of the electrical contacts which
results in a metal vapor arc. This arc is quickly extinguished
due to the insulating properties of vacuum.
46211 - Electrical apparatus for switching or protecting
CPC code electrical circuits, or for making connexions to or in electrical
circuits, for a voltage exceeding 1000 V
Independent verification of the declaration and data,
according to ISO 14025: 2010.
☐INTERNAL ☒ EXTERNAL
Independent verification
Independent verifier approved by EPD Norway: Anne Rønning
Signature:
Håkon Hauan, CEO EPD-Norge
Approved by
Signature:
Core PCR: EPDItaly007 – PCR for Electronic and Electrical
Reference PCR and version Products and Systems, Rev. 2, 2020/10/21.
number PCR: EPDItaly012 - Electronic and electrical products and
systems – Switches, Rev. 0, 2020/03/16.
EN 50693:2019 - Product category rules for life cycle
Core PCR assessments of electronic and electrical products and
systems.
Product RSL description 20 years
World (raw materials),
Markets of applicability Germany (production, use and end-of-life)
Europe (use and end-of-life)
STATUS SECURITY LEVEL DOCUMENT ID. REV. LANG. PAGE
Approved Public 3XAA008728 B001 EN 2/19
© Copyright 2022 ABB. All rights reserved.
ENVIRONMENTAL PRODUCT DECLARATION
This EPD is based on the LCA study described in the LCA
LCA study
report 3XAA008727
EPD type Product specific
EPD scope “Cradle to grave”
Year of reported primary data 2021
2B Srl (Italy)
Technical support
Via della Chiesa Campocroce 4, Mogliano Veneto (TV)
LCA software SimaPro 9.4.0.1 (2021)
LCI database ecoinvent v3.8 (2021)
LCIA methodology EN 50693:2019
EPDs published within the same product category, though
originating from different programs, may not be comparable.
Comparability Full conformance with a PCR allows EPD comparability only
when all stages of a life cycle have been considered. However,
variations and deviations are possible.
The owner of the declaration shall be liable for the underlying
information and evidence. EPD Norway shall not be liable with
Liability
respect to manufacturer, life cycle assessment data and
evidences.
Author of the life cycle Cemre Akdag – cemre.akdag@de.abb.com
assessment R&D Engineer
STATUS SECURITY LEVEL DOCUMENT ID. REV. LANG. PAGE
Approved Public 3XAA008728 B001 EN 3/19
© Copyright 2022 ABB. All rights reserved.
ENVIRONMENTAL PRODUCT DECLARATION
Contents
ABB Purpose & Embedding Sustainability ..................................................................................... 5
General Information ........................................................................................................................ 6
Constituent materials ..................................................................................................................... 8
LCA background information ........................................................................................................ 10
Inventory analysis .......................................................................................................................... 13
Environmental indicators .............................................................................................................. 15
Additional environmental information ........................................................................................ 17
References....................................................................................................................................... 18
STATUS SECURITY LEVEL DOCUMENT ID. REV. LANG. PAGE
Approved Public 3XAA008728 B001 EN 4/19
© Copyright 2022 ABB. All rights reserved.
ENVIRONMENTAL PRODUCT DECLARATION
ABB Purpose & Embedding Sustainability
ABB is a leading global technology company that energizes the transformation of society
and industry to achieve a more productive, sustainable future. By connecting software to
its electrification, robotics, automation and motion portfolio, ABB pushes the boundaries
of technology to drive performance to new levels. With a history of excellence stretching
back more than 130 years, ABB’s success is driven by about 110 thousand talented em-
ployees in over 100 countries.
ABB's Electrification business offers a wide-ranging portfolio of products, digital solu-
tions and services, from substation to socket, enabling safe, smart and sustainable elec-
trification. Offerings encompass digital and connected innovations for low and medium
voltage, including EV infrastructure, solar inverters, modular substations, distribution au-
tomation, power protection, wiring accessories, switchgear, enclosures, cabling, sensing
and control.
ABB is committed to continually promoting and embedding sustainability across its op-
erations and value chain, aspiring to become a role model for others to follow. With its
ABB Purpose, ABB is focusing on reducing harmful emissions, preserving natural re-
sources and championing ethical and human behavior.
STATUS SECURITY LEVEL DOCUMENT ID. REV. LANG. PAGE
Approved Public 3XAA008728 B001 EN 5/19
© Copyright 2022 ABB. All rights reserved.
ENVIRONMENTAL PRODUCT DECLARATION
General Information
The range of ABB Ratingen includes innovative and smart systems, with components and
services for power distribution and switching and control technology. The product range
of the Ratingen plant includes components such as vacuum interrupters, pole parts, cir-
cuit breakers, current limiters and core modules for the production of primary gas-insu-
lated switchgear. These components are widely used in associated plants within the
worldwide ABB value chain as well as by OEM partners in the industry.
ABB DE-ELDS adopts and implements for its own activities an integrated Quality/Environ-
mental/Health Management System in compliance with the following standards:
•UNI EN ISO 9001/2015 - Quality Management Systems- Requirements
•UNI EN ISO 14001/2015 – Environmental Management Systems – Requirements
•UNI EN ISO 45001:2018 - Occupational Health and Safety Management Systems
The VI type VG4-S declared in this EPD includes one main version within different applica-
tion cases, but all are covered with the same VI. This includes certain voltage levels (12 kV
/ 17.5 kV / 24 kV) and specific current levels for rated current (1250 A) and short-circuit
current (31.5 kA / 25 kA)
Technical information
Product Name VG4-S
Rated voltage [kV] 12 / 17.5 / 24
Rated current [A] 1250
Rated short circuit breaking current [kA] 25 / 31.5
Forming the heart of medium-voltage switchgear, vacuum interrupters (VIs) are an indis-
pensable part of the medium-voltage distribution network. As the core component for all
switching applications, VIs are widely used in utility power transmission systems, power
generation units, and power-distribution systems for railways, arc furnace applications,
and industrial plants. The main purpose of the vacuum interrupter is to establish or inter-
rupt a current flow by separation of the electrical contacts which results in a metal vapor
arc. This arc is quickly extinguished due to the insulating properties of the vacuum.
To increase external dielectric strength and to protect the vacuum interrupter from the
external influence it is embedded in silicone or epoxy resin or thermoplastic. The vacuum
interrupter itself cannot work stand-alone, it always requires additional outer protection
and terminal connection (pole part) and a mechanism to open the contacts (circuit
breaker). The vacuum interrupters are embedded in a special cast resin or thermoplastic
which makes the pole parts of the circuit-breaker notably robust and at the same time
protects the ABB vacuum interrupters from impact, dust, moisture and external damage.
The vacuum interrupter and the pole parts are maintenance-free products/components.
The whole system cannot work stand-alone, it requires a mechanical or electrical drive to
STATUS SECURITY LEVEL DOCUMENT ID. REV. LANG. PAGE
Approved Public 3XAA008728 B001 EN 6/19
© Copyright 2022 ABB. All rights reserved.
ENVIRONMENTAL PRODUCT DECLARATION
create a gap between the two contacts. With additional drive the system can be seen as
completed as a circuit breaker.
Vacuum circuit breakers are used in electrical distribution for control and protection of
cables, overhead lines, distribution substations, motors, transformers, generators and ca-
pacitor banks. The scope of the medium voltage circuit breakers is to interrupt an electric
current with a mechanical actuator (spring mechanism).
The manufacturing of the VI’s and pole parts is located in ABB Ratingen, where the vacuum
interrupters are assembled and produced. All components and some of the subassem-
blies are produced by ABB’s suppliers and are then assembled in the factory.
STATUS SECURITY LEVEL DOCUMENT ID. REV. LANG. PAGE
Approved Public 3XAA008728 B001 EN 7/19
© Copyright 2022 ABB. All rights reserved.
ENVIRONMENTAL PRODUCT DECLARATION
Constituent materials
The VG4-S part weights about 2.58 kg. All parts are included in the analysis.
Product weight
Materials Name CAS Number %
[kg]
Polyamide & Polybutylen-
--- 0.024 0.93
terephthalate glass filled
Plastics
Other plastics and rub-
--- --- ---
bers
Stainless Steel 65997-19-5 0.36 14.14
Copper 7440-50-8 1.79 69.49
Metals
Chromium 7440-47-3 0.08 3.1
Silver 7440-22-4 0.009 0.36
Ceramics 66402-68-4 0.31 11.95
Others
Others --- 0.0059 0.02
Total 2.58 100
VG4-S
Silver Plastics
0,36% 0,93%
Stainless Steel
14,14%
Other
0,02%
Ceramics
11,95%
Chromium
3,10%
Copper
69,49%
For the packaging small parts as sticking labels and grease, which are representing a
smaller fraction of the total mass, are neglected as their mass represents less than 2% of
that of the whole component, as stated in the paragraph of cut-off criteria of EPDItaly-
012: “Materials making up the switch itself whose total mass does not exceed 2% of the
total weight of the device”.
Scraps for metal working and plastic processes are included when already defined in
ecoinvent. The single-use packaging and reusable packaging are also included in the anal-
ysis in the manufacturing core stage. The packaging is common for VG4-S, it is composed
of steel fixing brackets, a cardboard box, and a wooden pallet, resulting in a total weight
STATUS SECURITY LEVEL DOCUMENT ID. REV. LANG. PAGE
Approved Public 3XAA008728 B001 EN 8/19
© Copyright 2022 ABB. All rights reserved.
ENVIRONMENTAL PRODUCT DECLARATION
of 27.7 kg for single-use box and 36.2 kg for reusable packaging with additional packaging
elements. ABB receives packaging components from outside suppliers and packages the
vacuum interrupter before shipping them.
STATUS SECURITY LEVEL DOCUMENT ID. REV. LANG. PAGE
Approved Public 3XAA008728 B001 EN 9/19
© Copyright 2022 ABB. All rights reserved.
ENVIRONMENTAL PRODUCT DECLARATION
LCA background information
Functional Unit
The functional unit of this study is to establish or interrupt the electrical continuity of a
circuit within a switchgear compartment in power systems during a reference service life
of 20 years.
The reference flow is a single vacuum interrupter including related accessories and pack-
aging.
System Boundaries
The life cycle of the vacuum interrupter VG4-S is a “from cradle to grave” analysis and co-
vers the following main life cycle stages: manufacturing, including the relevant upstream
process (e.g. acquisition of raw material, preparation of semi-finished goods, etc.) and
the main manufacturing and processing steps; distribution; installation, including the rel-
evant steps for the preparation of the product for use; use including the required mainte-
nance steps within the RSL (reference service life of the product) associated to the refer-
ence product; end-of-life stage, including the necessary steps until final disposal or
recovery of the product system.
The following table shows the stages of the product life cycle and the information stages
according to EN-50693 for the evaluation of electronic and electrical products and sys-
tems.
STATUS SECURITY LEVEL DOCUMENT ID. REV. LANG. PAGE
Approved Public 3XAA008728 B001 EN 10/19
© Copyright 2022 ABB. All rights reserved.
ENVIRONMENTAL PRODUCT DECLARATION
The stages of the product life cycle and the information considered for the evaluation of
the VG4-S are:
• Manufacturing upstream includes raw materials, and production activities of ABB
suppliers, including transport of semi-finished items and subassemblies to ABB
Ratingen site.
• The core part of the manufacturing stage includes local consumptions (ABB Rat-
ingen) the relevant assembling and waste due to manufacturing as well as the
packaging production.
• The distribution stage includes the impacts related to the distribution of the prod-
uct at the installation site.
• The installation stage includes the end of life of the packaging.
• The use and maintenance stages include the impact related to energy consump-
tion during the service life of the product.
• The end-of-life stage includes all activities related to waste treatment and dis-
posal of the product at the end of its service life.
Temporal and geographical boundaries
The ABB component suppliers are sourced all over the world. All primary data collected
from ABB are from 2021, which is a representative production year. Secondary data are
also representative for this year, as provided by ecoinvent v3.8.
The selected ecoinvent processes in the LCA model have global representativeness, due to
the unclear origin of each component. In this way, a conservative approach has been
adopted. The results of this study are only applicable to VG4-S vacuum interrupters pro-
duced in Ratingen in 2021.
Boundaries in the life cycle
As indicated in the PCR EPDItaly012, capital goods, such as buildings, machinery, tools
and infrastructure, the packaging for internal transport which cannot be allocated directly
to the production of the reference product, may be excluded from the system boundary.
Infrastructures, when present, such as processes deriving from the ecoinvent database
have not been excluded.
Data quality
In this EPD, both primary and secondary data are used. Site-specific foreground data have
been provided by ABB. The main data sources are the bill of materials available on the
enterprise resource planning. For all processes for which primary are not available, generic
data originating from the ecoinvent v3.8 database, allocation cut-off by classification, are
used. The ecoinvent database is available in the SimaPro 9.4.0.1 software used for the cal-
culations.
STATUS SECURITY LEVEL DOCUMENT ID. REV. LANG. PAGE
Approved Public 3XAA008728 B001 EN 11/19
© Copyright 2022 ABB. All rights reserved.
ENVIRONMENTAL PRODUCT DECLARATION
Environmental impact indicators
The information obtained from the inventory analysis is aggregated according to the ef-
fects related to the various environmental issues. According to PCR EPDItaly007 and
EN 50693 the environmental impact indicators must be determined using the characteri-
zation factors and impact assessment methods specified in
EN 15804:2012+A2:2019.
PCR EPDItaly007 and the EN 50693 standards establish four indicators for climate impact
(GWP-GHG): GWP (total) which includes all greenhouse gases; GWP (fossil fuels); GWP (bi-
ogenic carbon) which includes the emissions and absorption of biogenic carbon dioxide
and biogenic carbon stored in the product; GWP (land use and land use change).
Allocation rules
Allocation keys are used for consumptions related to the manufacturing process in the
production site as well as for company waste and product distribution. Since the factory
produces several products (components, apparatus and switchgears), only a part of the
environmental impact has been allocated to the specific production line. The values for
the electricity, heat, pressurized air, and water consumption have been read and recorded
from the counters which are distributed in the whole factory and are connected to certain
areas or even single machines or single workstations.
For the end-of-life allocation, the “polluter pays” principle is adopted according to what is
defined in the CEN/TR 16970 standard, as required by the PCR EPDItaly007. This means
that waste treatment processes are allocated to the product system that generates the
waste until the end-of-waste state is reached. The environmental burdens of recycling and
energy recovery processes are therefore allocated to the product system that generates
the waste, while the product system that uses the exported energy and recycled materials
receives it burden-free. However, the potential benefits and avoided loads from recovery
and recycling processes are not considered because it is not required by EPDItaly007.
Limitations and simplifications
The raw material life cycle stage includes the extraction of all raw materials. There is no
neglection of any components or materials within the analysis.
For the packaging small parts such as sticking labels and grease, which are representing
a smaller fraction of the total mass, are neglected as their mass represents less than 2%
of that of the whole component, as stated in the paragraph of the cut-off criteria of
EPDItaly-012: “Materials making up the switch itself whose total mass does not exceed 2%
of the total weight of the device”. Scraps for metal working and plastic processes are
included when already defined in ecoinvent.
STATUS SECURITY LEVEL DOCUMENT ID. REV. LANG. PAGE
Approved Public 3XAA008728 B001 EN 12/19
© Copyright 2022 ABB. All rights reserved.
ENVIRONMENTAL PRODUCT DECLARATION
Inventory analysis
In this LCA both primary and secondary data are used. Site-specific foreground data have
been provided by ABB. For data collection, Bills of Material (BOM) extracted from ABB's
internal SAP and PLM software were used. They are a list of all the components and
assemblies that constitute the finished product organized by level. Each item is matched
with its code, quantity, weight, and supplier. The BOMs were then processed, adding
material, surface area and other weight data taken from technical drawings. Finally, the
manufacturing process and surface treatment were assigned, according to information
provided by the R&D and Industrialization functions. Road distances between the
suppliers and ABB were calculated using Google Maps, and marine distances using
distances & time according to searates.com.
All primary data collected from ABB are from 2021 which was a representative production
year. The ecoinvent v3.8 cut-off by classification system processes are used to model the
background system of the processes.
The raw material inputs are modeled with data from ecoinvent representing a global
market coverage. These datasets are assumed to be representative.
Manufacturing stage
The vacuum interrupter is composed of several components all of which are made from
numerous materials. Most of the inputs to the products’ manufacturing stage are already
produced components. Copper is the most frequently used material followed by stainless
steel and ceramics.
The single-use packaging and reusable packaging are also included in the analysis in the
manufacturing core stage including all elements and components belonging to
packaging. ABB receives packaging components from outside suppliers and packages the
vacuum interrupter before shipping them.
The transport distances from raw materials suppliers to the manufacturing are not
known. However, this information is included in the data sets of ecoinvent “market for”.
The distance from the subassembly or single parts manufacturing factory to ABB facility
is calculated. In the factory, the different components and subassemblies are assembled
into the vacuum interrupter. All the components are produced by ABB’s suppliers.
The energy mix used for the production phase is representative for Ratingen production
site and includes an autonomous combined heat and power plant (CHP) driven by natural
gas.
Distribution
The transport distances from ABB plant to the place of use were exactly defined. There
are four customers identified. The reference port is Rotterdam, NL.
STATUS SECURITY LEVEL DOCUMENT ID. REV. LANG. PAGE
Approved Public 3XAA008728 B001 EN 13/19
© Copyright 2022 ABB. All rights reserved.
ENVIRONMENTAL PRODUCT DECLARATION
Installation
The installation phase only implies manual activities and no energy is consumed. This
phase also includes the disposal of the packaging of the VG4-S.
Use
Use and maintenance are modelled according to the PCR EPDItaly012 – Switches for the
VG4-S. As written in the PCR EPDItaly012 they are modelled according to the PCR
EPDItaly007 and EN_50593 . For the use phase, the general European medium voltage
electricity mix from ecoinvent v3.8 is used.
Since no maintenance happens during the use phase the environmental impacts linked to
this procedure have been omitted from the analysis. During the use phase, the VG4-S
dissipates some electricity due to ohmic losses. Electricity consumption was calculated
with the following formula:
P * 8760 * RSL * α
E [kWh]= use
use 1000
P =R*(0.5*I)2
use
α=0.3
with
• P =Power losses
use
• E =Energy losses
use
• RSL = Reference Service Lifetime
• R = Resistance
• I = Rated Current which is flowing through component during steady-state
• 8760 h = The number of hours in a year;
• α = Coefficient describing the amount of time in which the switch is requested
to operate its function
Parameters Values
Nominal current [A] 1250
RSL [Years] 20
α [%] 30
P [W] 3.52
use
E [kWh] 184.78
use
The RSL is adopted from the PCR EPDItaly012 with 20 years, the operational time and
power are assumed to be 30% for all the service life. Since no maintenance happens during
the use phase, the environmental impacts linked to this procedure are omitted from the
analysis.
End of life
The transport distances from the place of use to the place of disposal are assumed to be
100 km.
STATUS SECURITY LEVEL DOCUMENT ID. REV. LANG. PAGE
Approved Public 3XAA008728 B001 EN 14/19
© Copyright 2022 ABB. All rights reserved.
ENVIRONMENTAL PRODUCT DECLARATION
The end-of-life stage is modelled according to PCR EPDItaly012 and IEC/TR 62635. The
percentages for end-of-life treatments of circuit breakers are taken from IEC/TR 62635,
while the data for packaging waste scenarios are provided by EUROSTAT.
Environmental indicators
The following tables show the environmental impact indicators of the life cycle of a single
vacuum interrupter of type VG4-S, as indicated by PCR EPDItaly007, PCR EPDItaly012 and
EN 50693:2019.
The indicators are divided into the contribution of the processes to the different modules
(upstream, core and downstream) and stages (manufacturing, distribution, installation,
use and end-of-life).
UPSTREAM CORE DOWNSTREAM
Impact category Unit Total Distributi End of
Manufacturing Installation Use
on life
kg CO2
Climate change 1.25E+02 2.69E+01 2.18E+01 4.11E-01 5.02E-01 7.50E+01 5.20E-01
eq
Climate change - kg CO2
1.22E+02 2.64E+01 2.24E+01 4.11E-01 6.39E-02 7.24E+01 4.61E-01
Fossil eq
Climate change - kg CO2
2.67E+00 4.46E-01 -6.31E-01 1.04E-04 4.39E-01 2.36E+00 5.80E-02
Biogenic eq
Climate change -
kg CO2
Land use and Land 2.18E-01 4.47E-02 2.22E-03 2.53E-04 5.19E-05 1.71E-01 3.86E-04
eq
use change
kg
Ozone depletion CFC11 7.50E-06 1.65E-06 2.13E-06 8.68E-08 5.01E-09 3.59E-06 3.54E-08
eq
mol H+
Acidification 1.76E+00 1.33E+00 3.09E-02 9.86E-03 2.09E-04 3.90E-01 1.71E-03
eq
Eutrophication,
kg P eq 1.83E-01 1.10E-01 7.33E-04 1.73E-05 8.08E-06 7.25E-02 1.00E-04
freshwater
kg
Photochemical
NMVOC 4.96E-01 2.88E-01 3.78E-02 7.25E-03 2.14E-04 1.61E-01 1.39E-03
ozone formation
eq
Depletion of
abiotic resources
kg Sb eq 3.62E-02 3.60E-02 3.07E-05 6.83E-07 2.26E-07 1.70E-04 4.06E-06
– minerals and
metals
Depletion of
abiotic resources MJ 2.12E+03 3.27E+02 2.37E+02 5.63E+00 4.87E-01 1.54E+03 4.74E+00
– fossil fuels
Water use
m3 3.96E+01 2.20E+01 8.00E-01 1.34E-02 2.14E-03 1.68E+01 7.21E-02
(AWARE)
STATUS SECURITY LEVEL DOCUMENT ID. REV. LANG. PAGE
Approved Public 3XAA008728 B001 EN 15/19
© Copyright 2022 ABB. All rights reserved.
ENVIRONMENTAL PRODUCT DECLARATION
Resource use UPSTREAM CORE DOWNSTREAM
Unit Total
parameters Manufacturing Distribution Installation Use End of Life
PENRE MJ 2.12E+03 3.26E+02 2.34E+02 5.63E+00 4.88E-01 1.54E+03 4.74E+00
PERE MJ 3.50E+02 7.36E+01 9.01E+00 4.98E-02 2.14E-02 2.66E+02 3.39E-01
PENRM MJ 4.32E+00 1.41E+00 2.91E+00 0.00E+00 0.00E+00 0.00E+00 0.00E+00
PERM MJ 8.29E+00 0.00E+00 8.29E+00 0.00E+00 0.00E+00 0.00E+00 0.00E+00
PENRT MJ 2.12E+03 3.27E+02 2.37E+02 5.63E+00 4.88E-01 1.54E+03 4.74E+00
PERT MJ 3.58E+02 7.36E+01 1.73E+01 4.98E-02 2.14E-02 2.66E+02 3.39E-01
Net use of
fresh water m3 1.87E+00 5.55E-01 2.37E-02 4.49E-04 1.21E-04 1.29E+00 2.51E-03
(from AWARE)
Use of
secondary kg 1.80E-01 1.77E-01 3.51E-03 0.00E+00 0.00E+00 0.00E+00 0.00E+00
material
*PENRE: Use of non-renewable primary energy excluding non-renewable primary energy resources used as raw material; *PERE:
Use of renewable primary energy excluding renewable primary energy resources used as raw material; *PENRM: Use of non-
renewable primary energy resources used as raw material; *PERM: Use of renewable primary energy resources used as raw ma-
terial; *PENRT: Total use of non-renewable primary energy resources (primary energy and primary energy resources used as raw
materials) ;*PERT: Total use of renewable primary energy resources (primary energy and primary energy resources used as raw
materials)
UPSTREAM CORE DOWNSTREAM
Waste production
Unit Total End of
indicators Manufacturing Distribution Installation Use
life
Hazardous waste
kg 5.62E-03 4.71E-03 3.42E-04 8.22E-06 1.00E-06 5.48E-04 7.68E-06
disposed
Non-hazardous
kg 1.63E+01 9.90E+00 4.92E-01 1.96E-01 3.08E-02 5.11E+00 6.21E-01
waste disposed
Radioactive waste
kg 1.27E-02 1.10E-03 1.99E-04 3.87E-05 2.42E-06 1.13E-02 2.03E-05
disposed
Materials for
kg 4.41E-01 0.00E+00 1.41E-01 0.00E+00 2.83E-01 0.00E+00 1.69E-02
energy recovery
Materials for
kg 3.55E+00 5.01E-01 7.41E-01 0.00E+00 3.33E-01 0.00E+00 1.97E+00
recycling
Exported thermal
MJ 1.68E+00 0.00E+00 6.50E-01 0.00E+00 1.03E+00 0.00E+00 4.60E-04
Energy
Exported
MJ 8.42E-01 0.00E+00 3.29E-01 0.00E+00 5.13E-01 0.00E+00 2.35E-04
electricity energy
STATUS SECURITY LEVEL DOCUMENT ID. REV. LANG. PAGE
Approved Public 3XAA008728 B001 EN 16/19
© Copyright 2022 ABB. All rights reserved.
ENVIRONMENTAL PRODUCT DECLARATION
Additional environmental information
Reciclability potential
The recyclability potential of the reference product is calculated by dividing “MFR: material
for recycling” with the total weight of the vacuum interrupter This is based on the end-of-
life scenario adopted from IEC/TR 62635 Edition 1.0 which is representative for Europe.
The scenario is based on the rates given for materials that go through a separation pro-
cess, and the production losses in the recycling processes have also been considered;
thus, a conservative approach is adopted.
Recyclability potential
VG4-S 76.3 %
GHG emissions from the use of electricity in the manufacturing phase
The energy mix used for the production phase is representative for Ratingen production
site and includes an autonomous combined heat and power plant (CHP) driven by natural
gas.
Data source Amount Unit
kg CO2-
Ecoinvent 3.8 heat and power co-generation, natural gas 0.6015
eq/kWh
Dangerous substances
The product contains no substances given by the REACH Candidate list.
Indoor environment
The product meets the requirements for low emissions.
Carbon footprint
Carbon footprint has not been worked out for the product.
STATUS SECURITY LEVEL DOCUMENT ID. REV. LANG. PAGE
Approved Public 3XAA008728 B001 EN 17/19
© Copyright 2022 ABB. All rights reserved.
ENVIRONMENTAL PRODUCT DECLARATION
References
• Akdag, C. (2022) VG4_S: Life Cycle Assessment Report, Doc. no 3XAA008727, ABB
Switzerland Ltd, Group Technology ManagementEN 50693:2019 - Product cate-
gory rules for life cycle assessments of electronic and electrical products and
systems
• EN 15804:2012+A2:2019 – Sustainability of constructions – Environmental prod-
ucts declarations (September 2019)
• PCR EPDItaly007 - Electronic and electrical products and systems (rev.2), Octo-
ber 2020
• PCR EPDItaly012 - Electronic and electrical products and systems - Switches,
March 2020
• IEC/TR 62635 - Guidelines for end-of-life information provided by manufacturers
and recyclers and for recyclability rate calculation of electrical and electronic
equipment - Edition 1.0 2012-10
• UNI EN ISO 14040:2021 - Environmental management -Life cycle assessment -
Principles and framework
• UNI EN ISO 14044:2021 - Environmental management - Life cycle assessment -
Requirements and guidelines
• Ecoinvent, 2021. Swiss Centre for Life Cycle Assessment, v3.8
(www.ecoinvent.ch).
• PRé Consultants, 2021. Software SimaPro version 9.3.0.2 (www.pre.nl).
• https://ec.europa.eu/eurostat
• General Program Instructions for The Norwegian EPD Foundation/EPD-Norge
(www.epd-norge.no) version 5:2019
• EPDItaly Regulations rev. 5.2 (16/02/2022)
STATUS SECURITY LEVEL DOCUMENT ID. REV. LANG. PAGE
Approved Public 3XAA008728 B001 EN 18/19
© Copyright 2022 ABB. All rights reserved.
ENVIRONMENTAL PRODUCT DECLARATION
Program Operator and publisher Ph. +47 23 08 80 00
The Norwegian EPD Foundation
Post Box 5250 Majorstuen, 0303
email: post@epd-norge.no
Oslo
Norway web www.epd-norge.no
Owner of the declaration
ABB Switzerland Ltd, Group
Technology Management
Brown Boveri Straße 6, 5400 Baden,
web www.abb.com
Switzerland
Author of the life cycle assessment Ph. +49 170 4454877
Cemre Akdag
ABB AG email: cemre.akdag@de.abb.com
Oberhausener Str. 33, 40472
web www.abb.com
Ratingen, Germany
STATUS SECURITY LEVEL DOCUMENT ID. REV. LANG. PAGE
Approved Public 3XAA008728 B001 EN 19/19
© Copyright 2022 ABB. All rights reserved.
