Environmental product declaration
in accordance with ISO 14025 and EN 15804+A2
VDW
Owner of the declaration: Program operator:
TROX España The Norwegian EPD Foundation
Product: Declaration number:
VDW
NEPD-8761-8419
Declared unit:
1 pcs
Registration number:
This declaration is based on Product Category Rules:
NEPD-8761-8419
CEN Standard EN 15804:2012+A2:2019 serves as core
PCR Issue date: 16.01.2025
The Norwegian EPD Foundation NPCR 030:2021 Part B for ventilation components
Valid to: 16.01.2030
EPD software:
LCAno EPD generator ID: 556814
1 / 11
General information
Product Owner of the declaration:
VDW TROX España
Contact person:
Phone:
e-mail: arancha.salvador@troxgroup.com
Program operator: Manufacturer:
The Norwegian EPD Foundation TROX España
Post Box 5250 Majorstuen, 0303 Oslo, Norway
Phone: +47 977 22 020
web: www.epd-norge.no
Declaration number: Place of production:
TROX España
NEPD-8761-8419
Poligono Indstrial La Cartuja
E-50720 Zaragoza, Spain
This declaration is based on Product Category Rules: Management system:
CEN Standard EN 15804:2012+A2:2019 serves as core PCR
NPCR 030:2021 Part B for ventilation components
Statement of liability: Organisation no:
The owner of the declaration shall be liable for the underlying
information and evidence. EPD Norway shall not be liable with respect
to manufacturer information, life cycle assessment data and
evidences.​
Declared unit: Issue date:
1 pcs VDW
16.01.2025
Declared unit with option: Valid to:
A1-A3,A4,C1,C2,C3,C4,D 16.01.2030
Year of study:
2024
Functional unit: Comparability:
EPD of construction products may not be comparable if they not
comply with EN 15804 and seen in a building context.
General information on verification of EPD from EPD tools: Development and verification of EPD:
Independent verification of data, other environmental information The declaration is created using EPD tool lca.tools ver EPD2022.03,
and the declaration according to ISO 14025:2010, § 8.1.3 and § 8.1.4. developed by LCA.no. The EPD tool is integrated in the company's
Verification of each EPD is made according to EPD-Norway’s management system and has been approved by EPD Norway.
guidelines for verification and approval requiring that tools are i) NEPDT72
integrated into the company's environmental management system, ii)
the procedures for use of the EPD tool are approved by EPD-Norway, Developer of EPD: Carlos Caliz
and iii) the process is reviewed annually by an independent third
Reviewer of company-specific input data and EPD:​ Salvador Espinosa
party verifier. See Appendix G of EPD-Norway's General Programme
Aranzazu
Instructions for further information on EPD tools
Verification of EPD tool: Approved:
Independent third party verification of the EPD tool, background data
and test-EPD in accordance with EPDNorway's procedures and
guidelines for verification and approval of EPD tools.
Third party verifier:
Alexander Borg, Asplan Viak AS
(no signature required)
2 / 11
Product
Product description:
Ceiling swirl diffusers with circular and square front plate for a high number of air changes, with low sound power level for comfort zones, with
individually manually adjustable air control blades.
Product specification
Front made of sheet steel, with the possibility of a painted finish for air supply and extraction
For installations with constant and variable air flow
Compatible with any ceiling system, with the possibility of suspended installation
High induction, which leads to a rapid reduction in the temperature difference and air speed
Up to 35 air changes per hour with a row of several diffusers, minimum distance between diffusers of 0.9 m (between central points)
Ideal for comfort installations
Materials kg %
Metal - Galvanized Steel 1,32 86,88
Powder coating 0,07 4,69
Plastic - Acrylonitrile butadiene
0,13 8,42
styrene (ABS)
Total 1,52 100,00
Packaging kg %
Packaging - Cardboard 0,14 100,00
Total incl. packaging 1,66 100,00
Technical data:
Nominal sizes: 300, 400, 500, 600, 625, 825 mm
Minimum air flow rate, with ?tZ = –6 K: 7 – 99 l/s or 25 – 357 m³/h
Maximum air flow rate with LWA ? 50 dB(A): 80 – 470 l/s or 288 – 1692 m³/h
Temperature difference of the supplied air: –12 to +10 K
Connection port for circular duct networks in compliance with EN 1506 or EN 13180
Port with flange for lip seal (if lip seal is requested as an accessory)
Market:
Europe
Reference service life, product
20-25 Years
Reference service life, building or construction works
60 Years
LCA: Calculation rules
Declared unit:
1 pcs VDW
Cut-off criteria:
All major raw materials and all the essential energy is included. The production processes for raw materials and energy flows with very small
amounts (less than 1%) are not included. These cut-off criteria do not​ apply for hazardous materials and substances.
Allocation:
The allocation is made in accordance with the provisions of EN 15804. Energy, water and waste production in-house is allocated equally among all
products through mass allocation. Effects of primary production of recycled materials is allocated to the main product in which the material was
used. The recycling process and transportation of the material is allocated to this analysis.
Data quality:
Specific data for the product composition are provided by the manufacturer. The data represent the production of the declared product and were
collected for EPD development in the year of study. Background data is based on EPDs according to EN 15804 and different LCA databases. The
data quality of the raw materials in A1 is presented in the table below.
Materials Source Data quality Year
Metal - Galvanized Steel ecoinvent 3.6 Database 2020
Packaging - Cardboard ecoinvent 3.6 Database 2019
Plastic - Acrylonitrile butadiene styrene (ABS) ecoinvent 3.6 Database 2019
Powder coating ecoinvent 3.6 Database 2019
3 / 11
System boundaries (X=included, MND=module not declared, MNR=module not relevant)
Construction Beyond the system
Product stage Use stage End of life stage
installation stage boundaries
A1 A2 A3 A4 A5 B1 B2 B3 B4 B5 B6 B7 C1 C2 C3 C4 D
X X X X MND MND MND MND MND MND MND MND X X X X X
System boundary:
Declared unit with options: A1-A3, A4, C1, C2, C3, C4, D
Additional technical information:
Circular and square ceiling swirl diffusers for high room air change rates.
Nominal sizes 300, 400, 500, 600, 625, 825.
Volume flow rate range 7 - 470l/s or 25 -1692m³/h.
Diffuser face made of galvanised sheet steel, powder-coated.
For variable and constant volume flows.
For all types of ceiling systems, and with an extended border also suitable for freely suspended installation.
High induction results in a rapid reduction of the temperature difference and airflow velocity.
Very high room air change rate due to row arrangement with a minimum pitch distance of 0. 9 m.
Ideal for comfort zones.
Circular diffuser faces can be easily mounted without tools in a circular plenum box with horizontal spigot.
Optional equipment and accessories:
Exposed diffuser face available in RAL CLASSIC colours, air control blades in black or white.
Horizontal or vertical duct connection.
Square plenum box with cord-operated damper unit and pressure tap.
waR slairetam tropsnarT gnirutcafunaM tropsnarT ylbmessA e​sU ecnanetniaM riapeR tnemecalpeR tnemhsibrufeR lanoitarepO ygrene esu lanoitarepO esu retaw -eD noitcurtsnoc noitilomed tropsnarT etsaW gnissecorp lasopsiD -yrevoceR-esueR laitnetop-gnilcyceR
4 / 11
LCA: Scenarios and additional technical information
The following information describe the scenarios in the different modules of the EPD.
Capacity utilisation Value
Transport from production place to user (A4) Distance (km) Fuel/Energy Consumption Unit
(incl. return) % (Liter/tonne)
Truck, 16-32 tonnes, EURO 6 (km) 36,7 % 600 0,043 l/tkm 25,80
De-construction demolition (C1) Unit Value
Demolition of building per kg of ventilation
kg/DU 1,99
product (kg)
Capacity utilisation Value
Transport to waste processing (C2) Distance (km) Fuel/Energy Consumption Unit
(incl. return) % (Liter/tonne)
Truck, 16-32 tonnes, EURO 6 (km) 36,7 % 50 0,043 l/tkm 2,15
Waste processing (C3) Unit Value
Waste treatment per kg Hazardous waste,
kg 0,035
incineration (kg)
Waste treatment per kg Plastics, incineration (kg) kg 0,064
Materials to recycling (kg) kg 1,18
Disposal (C4) Unit Value
Landfilling of ashes from incineration per kg
kg 0,0067
Hazardous waste, from incineration (kg)
Waste, hazardous waste, to landfill (kg) kg 0,035
Landfilling of ashes from incineration of Plastics,
kg 0,0015
process per kg ashes and residues (kg)
Waste, plastic, mixture, to landfill (kg) kg 0,064
Waste, scrap steel, to landfill (kg) kg 0,13
Benefits and loads beyond the system
Unit Value
boundaries (D)
Substitution of electricity (MJ) MJ 0,000065
Substitution of thermal energy, district heating
MJ 0,00098
(MJ)
Substitution of primary steel with net scrap (kg) kg 0,27
5 / 11
LCA: Results
The LCA results are presented below for the declared unit defined on page 2 of the EPD document.
Environmental impact
Indicator Unit A1-A3 A4 C1 C2 C3 C4 D
GWP-total kg CO2 -eq 1,14E+01 1,62E-01 2,64E-03 1,35E-02 2,29E-01 1,85E-02 -2,98E-01
GWP-fossil kg CO2 -eq 1,12E+01 1,62E-01 2,63E-03 1,35E-02 2,29E-01 1,84E-02 -2,98E-01
GWP-biogenic kg CO2 -eq 1,40E-01 6,71E-05 4,94E-07 5,60E-06 2,04E-04 8,97E-06 -1,64E-04
GWP-luluc kg CO2 -eq 1,06E-02 5,77E-05 2,08E-07 4,81E-06 2,25E-05 6,77E-05 -1,34E-04
ODP kg CFC11 -eq 1,21E-06 3,67E-08 5,69E-10 3,06E-09 1,00E-08 1,00E-09 -4,26E-07
AP mol H+ -eq 9,39E-02 4,66E-04 2,76E-05 3,89E-05 1,38E-04 5,22E-05 -1,48E-03
EP-FreshWater kg P -eq 5,47E-04 1,30E-06 9,59E-09 1,08E-07 2,00E-06 3,78E-07 -1,83E-05
EP-Marine kg N -eq 1,26E-02 9,22E-05 1,22E-05 7,69E-06 3,20E-05 2,03E-05 -3,06E-04
EP-Terrestial mol N -eq 2,79E-01 1,03E-03 1,33E-04 8,60E-05 3,50E-04 1,39E-04 -3,13E-03
POCP kg NMVOC -eq 4,31E-02 3,95E-04 3,67E-05 3,29E-05 9,52E-05 5,69E-05 -1,49E-03
ADP-minerals&metals1 kg Sb-eq 5,78E-03 4,48E-06 4,04E-09 3,73E-07 3,16E-07 5,87E-08 -5,14E-06
ADP-fossil1 MJ 1,65E+02 2,45E+00 3,63E-02 2,04E-01 3,57E-01 1,30E-01 -2,51E+00
WDP1 m3 7,86E+02 2,37E+00 7,70E-03 1,98E-01 1,33E+00 5,75E-01 1,54E+01
GWP-total = Global Warming Potential total; GWP-fossil = Global Warming Potential fossil fuels; GWP-biogenic = Global Warming Potential biogenic; GWP-luluc =
Global Warming Potential land use and land use change; ODP = Depletion potential of the stratospheric ozone layer; AP = Acidification potential, Accumulated
Exceedance; EP-freshwater = Eutrophication potential, fraction of nutrients reaching freshwater end compartment: EP-marine = Eutrophication potential, fraction of
nutrients reaching marine end compartment; EP-terrestrial = Eutrophication potential, Accumulated Exceedance; POCP = Formation potential of tropospheric ozone;
ADP-minerals&metals = Abiotic depletion potential for non-fossil resources; ADP-fossil = Abiotic depletion for fossil resources potential; WDP = Water (user)
deprivation potential, deprivation-weighted water consumption
"Reading example: 9,0 E-03 = 9,0*10-3 = 0,009"
*INA Indicator Not Assessed
1. The results of this environmental impact indicator shall be used with care as the uncertainties on these results are high or as there is limited experienced with the
indicator
Remarks to environmental impacts
6 / 11
Additional environmental impact indicators
Indicator Unit A1-A3 A4 C1 C2 C3 C4 D
PM Disease incidence 8,03E-07 9,93E-09 7,29E-10 8,28E-10 1,90E-09 9,07E-10 -2,47E-08
IRP2 kgBq U235 -eq 6,19E-01 1,07E-02 1,55E-04 8,93E-04 1,61E-03 3,50E-04 1,07E-03
ETP-fw1 CTUe 3,06E+02 1,82E+00 1,98E-02 1,52E-01 2,00E+00 2,82E-01 -1,66E+01
HTP-c1 CTUh 3,97E-08 0,00E+00 0,00E+00 0,00E+00 8,80E-11 3,60E-11 -1,43E-09
HTP-nc1 CTUh 5,08E-07 1,99E-09 1,80E-11 1,66E-10 7,23E-10 3,32E-10 3,11E-08
SQP1 dimensionless 5,22E+01 1,72E+00 4,60E-03 1,43E-01 1,36E-01 3,73E-01 -1,88E-01
PM = Particulate Matter emissions; IRP = Ionizing radiation – human health; ETP-fw = Eco toxicity – freshwater; HTP-c = Human toxicity – cancer effects; HTP-nc =
Human toxicity – non cancer effects; SQP = Potential Soil Quality Index (dimensionless)
"Reading example: 9,0 E-03 = 9,0*10-3 = 0,009"
*INA Indicator Not Assessed
1. The results of this environmental impact indicator shall be used with care as the uncertainties on these results are high or as there is limited experienced with the
indicator
2. This impact category deals mainly with the eventual impact of low dose ionizing radiation on human health of the nuclear fuel cycle. It does not consider effects due
to possible nuclear accidents, occupational exposure nor due to radioactive waste disposal in underground facilities. Potential ionizing radiation from the soil, from
radon and from some construction materials is also not measured by this indicator.
7 / 11
Resource use
Indicator Unit A1-A3 A4 C1 C2 C3 C4 D
PERE MJ 3,02E+01 3,51E-02 1,96E-04 2,93E-03 6,24E-02 3,20E-02 -2,04E-01
PERM MJ 0,00E+00 0,00E+00 0,00E+00 0,00E+00 0,00E+00 0,00E+00 0,00E+00
PERT MJ 3,02E+01 3,51E-02 1,96E-04 2,93E-03 6,24E-02 3,20E-02 -2,04E-01
PENRE MJ 1,59E+02 2,45E+00 3,63E-02 2,04E-01 3,57E-01 1,30E-01 -2,51E+00
PENRM MJ 5,89E+00 0,00E+00 0,00E+00 0,00E+00 -5,89E+00 0,00E+00 0,00E+00
PENRT MJ 1,65E+02 2,45E+00 3,63E-02 2,04E-01 -5,53E+00 1,30E-01 -2,51E+00
SM kg 1,20E+00 0,00E+00 1,78E-05 0,00E+00 0,00E+00 7,70E-04 0,00E+00
RSF MJ 6,33E-01 1,26E-03 4,82E-06 1,05E-04 1,38E-03 1,13E-04 1,08E-02
NRSF MJ 2,98E+00 4,49E-03 7,10E-05 3,74E-04 0,00E+00 7,01E-03 3,13E-01
FW m3 1,33E-01 2,62E-04 1,87E-06 2,19E-05 3,52E-04 1,10E-04 -6,27E-04
PERE = Use of renewable primary energy excluding renewable primary energy resources used as raw materials; PERM = Use of renewable primary energy resources used
as raw materials; PERT = Total use of renewable primary energy resources; PENRE = Use of non renewable primary energy excluding non-renewable primary energy
resources used as raw materials; PENRM = Use of non renewable primary energy resources used as raw materials; PENRT = Total use of non renewable primary energy
resources; SM = Use of secondary materials; RSF = Use of renewable secondary fuels; NRSF = Use of non-renewable secondary fuels; FW = Net use of fresh water
"Reading example: 9,0 E-03 = 9,0*10-3 = 0,009"
*INA Indicator Not Assessed
8 / 11
End of life - Waste
Indicator Unit A1-A3 A4 C1 C2 C3 C4 D
HWD kg 8,24E-02 1,26E-04 1,07E-06 1,05E-05 0,00E+00 3,57E-02 -1,55E-03
NHWD kg 2,92E+00 1,19E-01 4,29E-05 9,94E-03 3,57E-02 2,03E-01 -1,22E-01
RWD kg 5,55E-04 1,67E-05 2,52E-07 1,39E-06 0,00E+00 9,72E-08 8,21E-07
HWD = Hazardous waste disposed; NHWD = Non-hazardous waste disposed; RWD = Radioactive waste disposed
"Reading example: 9,0 E-03 = 9,0*10-3 = 0,009"
*INA Indicator Not Assessed
End of life - Output flow
Indicator Unit A1-A3 A4 C1 C2 C3 C4 D
CRU kg 0,00E+00 0,00E+00 0,00E+00 0,00E+00 0,00E+00 0,00E+00 0,00E+00
MFR kg 3,77E-01 0,00E+00 1,75E-05 0,00E+00 1,19E+00 5,74E-06 0,00E+00
MER kg 7,19E-02 0,00E+00 5,42E-08 0,00E+00 3,57E-02 1,40E-07 0,00E+00
EEE MJ 4,82E-02 0,00E+00 1,86E-07 0,00E+00 3,53E-05 9,11E-06 0,00E+00
EET MJ 7,30E-01 0,00E+00 2,81E-06 0,00E+00 5,34E-04 1,38E-04 0,00E+00
CRU = Components for re-use; MFR = Materials for recycling; MER = Materials for energy recovery; EEE = Exported energy electrical; EET = Exported energy thermal
"Reading example: 9,0 E-03 = 9,0*10-3 = 0,009"
*INA Indicator Not Assessed
Biogenic Carbon Content
Indicator Unit At the factory gate
Biogenic carbon content in product kg C 0,00E+00
Biogenic carbon content in accompanying packaging kg C 0,00E+00
Note: 1 kg biogenic carbon is equivalent to 44/12 kg CO2
9 / 11
Additional requirements
Greenhouse gas emissions from the use of electricity in the manufacturing phase
National production mix from import, low voltage (production of transmission lines, in addition to direct emissions and losses in grid) of applied
electricity for the manufacturing process (A3).
Electricity mix Source Amount Unit
Electricity, low voltage, photovoltaic, roof installation, single-Si, panel, mounted (kWh) - Spain ecoinvent 3.6 72,70 g CO2-eq/kWh
Dangerous substances
The product contains no substances given by the REACH Candidate list.
Indoor environment
Additional Environmental Information
Additional environmental impact indicators required in NPCR Part A for construction products
Indicator Unit A1-A3 A4 C1 C2 C3 C4 D
GWPIOBC kg CO2 -eq 1,14E+01 1,62E-01 2,64E-03 1,35E-02 2,29E-01 1,87E-02 -4,46E-01
GWP-IOBC: Global warming potential calculated according to the principle of instantaneous oxidation. In order to increase the transparency of biogenic carbon​
contribution to climate impact, the indicator GWP-IOBC is required as it declares climate impacts calculated according to the principle of instantaneous oxidation.​
GWP-IOBC is also referred to as GWP-GHG in context to Swedish public procurement legislation.
10 / 11
Bibliography
ISO 14025:2010 Environmental labels and declarations - Type III environmental declarations - Principles and procedures.
ISO 14044:2006 Environmental management - Life cycle assessment - Requirements and guidelines.
EN 15804:2012+A2:2019 Environmental product declaration - Core rules for the product category of construction products.
ISO 21930:2017 Sustainability in buildings and civil engineering works - Core rules for environmental product declarations of construction
products.
ecoinvent v3, Allocation, cut-off by classification, Swiss Centre of Life Cycle Inventories.
Iversen et al., (2021) eEPD v2021.09 Background information for EPD generator tool system verification, LCA.no Report number: 07.21
Graafland and Iversen (2022) EPD generator for NPCR 030 Ventilation components, Background information for EPD generator application and
LCA data, LCA.no report number: 12.22
NPCR Part A: Construction products and services. Ver. 2.0. April 2021, EPD-Norge.
NPCR 030 Part B for Ventilation components, Ver. 1.0, 18.05.2021, EPD Norway.
ISO 14025:2010 Environmental labels and declarations - Type III environmental declarations - Principles and procedures.
ISO 14044:2006 Environmental management - Life cycle assessment - Requirements and guidelines.
EN 15804:2012+A2:2019 Environmental product declaration - Core rules for the product category of construction products.
ISO 21930:2017 Sustainability in buildings and civil engineering works - Core rules for environmental product declarations of construction
products.
ecoinvent v3, Allocation, cut-off by classification, Swiss Centre of Life Cycle Inventories.
Iversen et al., (2021) eEPD v2021.09 Background information for EPD generator tool system verification, LCA.no Report number: 07.21
Graafland and Iversen (2022) EPD generator for NPCR 030 Ventilation components, Background information for EPD generator application and
LCA data, LCA.no report number: 12.22
NPCR Part A: Construction products and services. Ver. 2.0. April 2021, EPD-Norge.
NPCR 030 Part B for Ventilation components, Ver. 1.0, 18.05.2021, EPD Norway.
EN ISO 9001:2015 - Quality management systems.
EN ISO 14001:2015 - Environmental management systems.
EN ISO 50001:2018 - Energy management systems.
Program operator and publisher Phone: +47 977 22 020
The Norwegian EPD Foundation e-mail: post@epd-norge.no
Post Box 5250 Majorstuen, 0303 Oslo, Norway web: www.epd-norge.no
Owner of the declaration: Phone:
TROX España e-mail: arancha.salvador@troxgroup.com
Poligono Indstrial La Cartuja, E-50720 Zaragoza, Spain web: https://www.trox.es/
Author of the Life Cycle Assessment Phone: +47 916 50 916
LCA.no AS e-mail: post@lca.no
Dokka 6A, 1671 Kråkerøy, Norway web: www.lca.no
Developer of EPD generator Phone: +47 916 50 916
LCA.no AS e-mail: post@lca.no
Dokka 6A, 1671 Kråkerøy, Norway web: www.lca.no
ECO Platform web: www.eco-platform.org
ECO Portal web: ECO Portal
11 / 11
