ENVIRONMENTAL PRODUCT DECLARATION
as per ISO 14025 and EN 15804+A2
Owner of the Declaration VELUX Group
Publisher Institut Bauen und Umwelt e.V. (IBU)
Programme holder Institut Bauen und Umwelt e.V. (IBU)
Declaration number EPD-VEL-20220135-IBJ3-EN
Issue date 25.07.2022
Valid to 24.07.2027
VELUX soft shutter - solar-powered
VELUX A/S
www.ibu-epd.com | https://epd-online.com
1. General Information
VELUX A/S VELUX soft shutter - solar-powered
Programme holder Owner of the declaration
IBU – Institut Bauen und Umwelt e.V. VELUX Group
Hegelplatz 1 Ådalsvej 99
10117 Berlin 2970 Hørsholm
Germany Denmark
Declaration number Declared product / declared unit
EPD-VEL-20220135-IBJ3-EN The declaration represents 1 m2 of the solar-powered VELUX soft shutter
SSS of the size MK06 = area of 0.91884 m2 (0.78 m*1.178 m). Being the
most sold product of this product family the declared values are also
representative for the VELUX soft shutter SSSS of the same size.
This declaration is based on the product category rules: Scope:
Sun protection systems, 01.08.2021 The declaration covers 100% of solar-powered VELUX soft shutters SSS
(PCR checked and approved by the SVR) and SSSS produced by KH-SK France S.A.S, France and by Gåsdal
Bygningsindustri A/S, Denmark.
The owner of the declaration shall be liable for the underlying information
Issue date and evidence; the IBU shall not be liable with respect to manufacturer
information, life cycle assessment data and evidences.
25.07.2022
The EPD was created according to the specifications of EN 15804+A2. In
the following, the standard will be simplified as EN 15804.
Valid to
24.07.2027 Verification
The standard EN 15804 serves as the core PCR
Independent verification of the declaration and data according to ISO
14025:2011
internally X externally
Dipl.-Ing. Hans Peters
(Chairman of Institut Bauen und Umwelt e.V.)
Florian Pronold Dr. Eva Schmincke,
(Managing Director Institut Bauen und Umwelt e.V.) (Independent verifier)
1 Environmental Product Declaration - VELUX A/S - VELUX soft shutter - solar-powered
2. Product
treated product as defined by the (EU) Regulation on Biocidal
2.1 Product description/Product definition Products No. 528/2012):
The Velux solar powered soft shutters SSS and SSSS are
• no
exterior shutters to be installed in connection with a VELUX roof
Recycled content
window. For the placing on the market of the product in the
European Union/European Free Trade Association (EU/EFTA)
(with the exception of Switzerland) Regulation (EU) No.
305/2011 (CPR) applies. The product needs a declaration of
performance taking into consideration EN
13561:2004+A1:2008, External blinds – Performance
requirements including safety and the CE-marking. For the
The values stated in the table relate to the recycled material
application and use the respective national provisions apply.
streams in VELUX production.
2.2 Application
VELUX shutters are installed on the exterior side of a VELUX 2.6 Manufacture
roof window, in connection with home improvement, renovation
Extruded aluminum profiles, aluminum coils, rubber and plastic
and new build.
are produced outside Velux.
2.3 Technical Data
The production and final assembly of shutters takes place in
The Declaration of Performance including relevant technical
the production sites in Denmark and France.
specifications and test methods/test standards can be
downloaded from the website www.velux.com/ce
The final production processes include shortening of extruded
Constructional data profiles, aluminum coils, cutting, drilling, rollforming of
Name Value Unit aluminum band, mounting of rubber gasket, brackets as well as
Resistance to wind load according to EN 13561 3 - packaging and stacking, wrapping on pallets.
Performance data of the product in accordance with the
The factories are ISO 9001 certified.
declaration of performance with respect to its essential
characteristics according to 2.7 Environment and health during manufacturing
• EN 13561:2004+A1:2008, External blinds – All factories are ISO 14001 and ISO 45001 certified.
Performance requirements including safety.
2.8 Product processing/Installation
2.4 Delivery status The factory-assembled product is installed on-site on the pre-
Soft shutters are manufactured ready for installation in installed window, by use of a screw driver. The solar panel is
predefined sizes, which are available for installation on most installed in the products as described in the installation guide,
VELUX windows types and within the majority of the window by which no afterward connection to the power grid is required.
size range.
2.9 Packaging
2.5 Base materials/Ancillary materials The packaging usually consists of:
Composition of the soft shutter SSS: • polyethylene film
Aluminium 65 % • cardboard
Motor (see below) 10 % • paper inserts
PVC coated polyester cloth with The use of other packaging materials is possible, but
acrylate on top 5 % insignificant in terms of quantity.
PC- PBT 3 %
TPV 2 % The plastic packaging (polyethylene (PE) film as well as the
PA 2 % cardboard and paper can be recycled if separated by type;
others alternatively, they can be incinerated.
Composition of the corresponding motor SSS: 2.10 Condition of use
Battry 35 % The material composition of VELUX soft shutters does not
DC motor 25 % change over their service life.
Aluminium 15 %
PA 6,6 w glass fibre 60% 15 % 2.11 Environment and health during use
others VELUX soft shutters do not contain any pollutants that could be
released during use.
1) This product/article/at least one partial article contains
substances listed in the candidate list (date: 02.03.2022) Environmental protection: According to current knowledge,
exceeding 0.1 percentage by mass: hazards to water, air and soil cannot arise when the products
are used as intended.
• no
2) This product/article/at least one partial article contains other
Health protection: According to current knowledge, no health
CMR substances in categories 1A or 1B which are not on the
hazards or impairments are to be expected.
candidate list, exceeding 0.1 percentage by mass:
• not investigated with suppliers 2.12 Reference service life
3) Biocide products were added to this construction product or it It is not possible to calculate the reference service life
has been treated with biocide products (this then concerns a according to ISO 15686. The reference service life based on a
2 Environmental Product Declaration - VELUX A/S - VELUX soft shutter - solar-powered
manufacturer's declaration is 30 years. The corresponding VELUX soft shutters can be dismantled manually without any
utilization scenario is declared in 4. The products are designed problems. The metal parts are usually recycled; the plastic
for outdoor use; external influences on the ageing of the parts are sent for thermal recycling for energy recovery.
product are minimal.
2.15 Disposal
2.13 Extraordinary effects VELUX soft shutters are mostly inert and can be disposed of in
Fire an appropriate landfill. However, due to the value of the
Product not tested according to EN 13501 under the CE-mark. materials or the carbon content of the plastic parts, recycling or
Water energy recovery is preferable and common.
In the event of unforeseen exposure to water (flood), the
electronic parts of VELUX soft shutters must be replaced as Waste code according to European Waste List (Regulation on
electrical components; no adverse effects on human health or the European Waste List):
the environment are to be expected.
16 02 14 electronic parts
Mechanical destruction 17 02 03 plastics
In the event of unforeseen mechanical destruction, VELUX soft 17 04 14 mixed metals
shutters must be replaced; no adverse effects on human health
or the environment are to be expected. 2.16 Further information
Further documentation on the products, technical data sheets,
2.14 Re-use phase BIM files, etc. can be found at:
www.velux.com
3. LCA: Calculation rules
under consideration or no significant environmental impacts
3.1 Declared Unit occur.
The declared unit is 1 m2 of the solar driven VELUX soft shutter
SSS of the size MK06 = area of 0.91884 m2 (0.78 m*1.178 m). Module B2 includes the one-time replacement of the motor
Being the most sold product of this product family and due to over the service life after 15 years. Since the composition and
minimal differences in the bill of materials, the declared values content of recyclate for the electric motor is not known, it is not
are also representative for the VELUX soft shutter SSSS of the considered for the calculation of module D.
same size.
Module B6 includes the electricity consumption for opening
Declared unit
and closing the soft shutters over their service life.
Name Value Unit
Declared unit 1 m2 Module C1 includes manual dismantling, with no significant
Grammage 9.72 kg/m2 environmental impact.
Module C2 comprises the transport of the dismantled VELUX
soft shutter to a sorting plant and then to a waste incineration
3.2 System boundary
plant for the thermally treated plastic fraction.
Type of EPD: Cradle to gate with options, with modules C1 –
C4, and module D (A1-A3, C1-C3, D and additional modules
Modules C3/C4: Given the complexity of the inventoried
products, a mixed end-of-life scenario is modelled, allowing the
The production of VELUX soft shutters (modules A1-A3)
different materials to follow their most likely path.
includes raw material extraction, energy generation, waste
As a rule of thumb, metals are recycled, and plastics are
treatment and all transports up to the factory gate. In
incinerated (also due to the very limited data availability of
accordance with COUNCIL REGULATION (EU) No 333/2011,
plastics recycling and its benefits).
secondary metals are modeled as part of the product system
from the moment they are available as unmixed scrap.
It is assumed that metals reach an end-of-waste state after
Waste or secondary fuels are not used for production.
having been sorted and transported to a recycler. The
combustible material (plastics) is assumed to be thermally
Module A4 is not declared due to large variances in transport
treated in a municipal waste incineration plant.
distances between the production site and the construction site,
where the product is installed.
Module D includes the benefits and burdens associated with
recycling metals beyond the system boundary, resulting from
Module A5: The products are delivered to the construction site
the treatment of recycled materials from the point of end-of-
ready to be installed. Manual installation is assumed, and
waste to the point of substitution (as loads) and substitution of
electricity consumption related to electric drilling machines,
primary resources (as benefits).
screw drivers, etc. is considered to be negligible. The
It also includes the benefits and burdens associated with
combustible packaging material (PE-foil) is assumed to be
energy recovery from plastic waste in a municipal waste
thermally treated in a municipal waste incineration plant with an
incineration (MWI) plant, as modeled in Module C3.
efficiency R1 < 0.6 (according to the ecoinvent dataset used);
In Module D, only net flows of metals leaving the product
the recovered energy is declared as exported energy.
system are considered.
Cardboard and paper are recycled; it is assumed that these
fractions reach the end-of-waste state after having been sorted 3.3 Estimates and assumptions
and transported (as a conservative choice) to a recycler. No
No further assumptions and estimates relevant to the result had
packaging waste is landfilled.
to be made beyond the points made in this chapter 3 and in
chapter 4.
Modules B1, B3 to B5 and B7 are not relevant for the product
3 Environmental Product Declaration - VELUX A/S - VELUX soft shutter - solar-powered
3.4 Cut-off criteria 3.8 Geographic Representativeness
No data available from the company survey was neglected. Land or region, in which the declared product system is
These include, among other things, material use, energy manufactured, used or handled at the end of the product´s
demand (heat, electricity), packaging materials of raw materials lifespan: Europe
(insofar as they are generated as waste) and product
packaging, consumables in production, waste treatment and
3.9 Allocation
the transport of all inputs and outputs.
With this approach, mass and energy flows below 1 % were No co-products are generated during the production of the
also accounted for. No processes were neglected that would VELUX products. Sorted production scrap of the different
have been known to the project managers and would have metals, notably aluminium, is considered a secondary material
contributed significantly to the indicators of the impact with no economic value (so no burdens allocated) and
assessment. considered in the quantification of net flows leaving the product
system. This approach is chosen to ensure a coherent
3.5 Background data quantification of net flows entering module D.
Ecoinvent 3.8 (2021) is used as the background database. No processes were modelled as part of the foreground model
that would have required an allocation of multi-input processes.
3.6 Data quality Background datasets on municipal waste incineration plants
The foreground data are based on extensive and detailed data were taken from ecoinvent without any modification.
collection at the production sites. The foreground data could be
fully linked with corresponding data records from the Allocation of reuse, recycling and recovery was avoided by the
background database ecoinvent 3.8. cut-off approach in the foreground model in line with DIN EN
The background data was updated in 2021. Thus, the quality of 15804.
the foreground and background data can be rated as very
good. 3.10 Comparability
Basically, a comparison or an evaluation of EPD data is only
3.7 Period under review possible if all the data sets to be compared were created
The LCA data represents the production conditions for the year according to EN 15804 and the building context, respectively
2021. the product-specific characteristics of performance, are taken
into account.
4. LCA: Scenarios and additional technical information
Characteristic product properties of biogenic carbon No packaging waste is landfilled.
Information on describing the biogenic carbon content at The use of multi-way pallets is not taken into account as
factury gate packaging material.
Name Value Unit
Reference service life
kg
Biogenic carbon content in product 0.0745
C
Biogenic carbon content in accompanying kg
0.741
packaging C
Note: 1 kg of biogenic carbon is equivalent to 44/12 kg of CO .
2
Module A5
The products are delivered to the construction site ready to be
installed. Manual installation is assumed, and electricity
consumption related to electric drilling machines, screw drivers,
etc. is considered to be negligible.
The combustible packaging material (plastics) is assumed to be
transported 50 km with a lorry 16-32 metric ton, EURO6 to an
incineration plant with an efficiency R1 < 0.6 (according to the
ecoinvent dataset used); the recovered energy is declared as
exported energy; for its quantification an efficiency of 25.6 % is
assumed for the production of heat and 13.0 % for the
production of electricity (always referring to the lower heating
value of the waste).
Metals, cardboard and paper are recycled; it is assumed that
these fractions reach the end-of-waste state after having been
sorted and transported (as a conservative choice) to a recycler
over 150 km with a lorry 16-32 metric ton, EURO6.
4 Environmental Product Declaration - VELUX A/S - VELUX soft shutter - solar-powered
Name Value Unit Manual de-installation is assumed, and electricity consumption
related to electric screw drivers, etc. is considered to be
Reference service life
negligible. Thus, no environmental impacts are declared in
according to
30 a module C1.
manufacturer's
declaration
Module C2
The product has passed
Declared product Given the complexity of the inventoried products, a mixed end-
internal quality controls and
properties (at the gate) - of-life scenario is modelled, allowing the different materials to
complies with EN 13659 for CE
and finishes follow their most likely path.
marking
Design application
It should also be noted that the deconstruction and waste
parameters (if instructed
treatment scenario can vary a lot, depending on the actual
by the manufacturer), Installation according to
situation. Thus, a generic end-of-life scenario is assumed.
including the references assembly instructions and -
to the appropriate state of the art.
As a rule of thumb, metals are recycled and plastics are
practices and application
incinerated (also due to the very limited data availability of
codes
plastics recycling and its benefits). The combustible material
An assumed quality of (plastics) is assumed to be transported 50 km with a lorry 16-32
work, when installed in metric tons, EURO6 to an incineration plant. Metals are
Carried out in accordance with
accordance with the - recycled; it is assumed that these fractions reach the end-of-
the manufacturer's instructions.
manufacturer’s waste state after having been sorted and transported to a
instructions recycler over 150 km with a lorry 16-32 metric tons, EURO6.
Outdoor environment, (for The declared products are
outdoor applications), e.g. intended for installation outside Module C3
weathering, pollutants, UVthe building: They are therefore A consumption of 0.03 kWh/kg of electricity for shredding and
-
and wind exposure, designed to withstand outdoor sorting and 0.437 MJ/kg of diesel fuel for internal logistics are
building orientation, conditions throughout their taken into account to disassemble the product. The recovered
shading, temperature service life. material leaves the product system as 'materials for recycling'.
Indoor environment (for The net amounts of the metals leaving the product system are
indoor applications), e.g. The declared products are not considered as 'use of secondary material' in Module D.
intended for installation inside -
temperature, moisture,
chemical exposure a building. Module C4
As stated above, it is assumed that 100% of the plastic parts
Usage conditions, e.g. Standard use in any type of
are treated in a waste incineration plant with an efficiency R1
frequency of use, building, i.e. opening/closing -
< 0.6 (according to the ecoinvent dataset used); 25.57% of the
mechanical exposure as often as necessary.
lower heating value of the plastic parts are recovered as heat
The declared products are
and 13.0% as electricity. Recovered energy is reported as
designed for a reference life of
Maintenance e.g. required 'exported energy' and considered in Module D.
30 years, with the motor
frequency, type and
replaced every 15 years. They -
quality and replacement Some of the material, notably laminated flat glass is assumed
are maintained by cleaning
of components to be landfilled.
water at the discretion of the
building occupants.
Module D
Module B1 Module D contains the benefits and loads beyond the system
The products are assumed to have no direct emissions during boundary related to the recycling of metals, which result from
the use phase. The indicator values of Module B1 are thus 0. the treatment of recycled materials from the point of end-of-
The soft shutters store minimal quantities of biogenic carbon. waste status to the point of substitution (as loads) and the
substitution of primary resources (as benefits).
Module B2
The maintenance scenario (B2) covers the replacement of the It also includes the benefits and loads related to the energy
motor over the service life of the product. Given that the recovery from plastic wastes in a MWIP as modelled in
detailed composition of the motor and its electronic Modules A3, A5 and C3.
components is not known, potential loads and benefits related
to the motor and electronics are disregarded. The benefits of the recycling of the motor and electronic parts
are not considered due to the absence of data on its
Annual cleaning with water (e.g., using 1 l/m2 of tap water per composition and recycled content.
annual cleaning) is neglected.
Due to a lack of data for plastics from de-construction activities,
Module B6 the substitution potential of recycled plastics is not taken into
For motor-operated soft shutters, electricity is used both on account.
stand-by and during the opening/closing cycles.
Only net flows leaving the product system are considered in
Module C1 module D.
5 Environmental Product Declaration - VELUX A/S - VELUX soft shutter - solar-powered
5. LCA: Results
Disclaimer:
EP-freshwater: This indicator has been calculated as 'kg P eq' as required in the characterization model (EUTREND model, Struijs et
al., 2009b, as implemented in ReCiPe; http://eplca.jrc.ec.europa.eu/LCDN/developerEF.xhtml)
DESCRIPTION OF THE SYSTEM BOUNDARY (X = INCLUDED IN LCA; MND = MODULE OR INDICATOR NOT DECLARED; MNR
= MODULE NOT RELEVANT)
Benefits and
Construction loads beyond
Product stage Use stage End of life stage
process stage the system
boundaries
la ire ta m w a Ry lp p u s tro p s n a rT g n iru tc a fu n a M e h t m o rf tro p s n a rTe tis e h t o t e ta g y lb m e s s A e s U e c n a n e tn ia M ria p e R tn e m e c a lp e R tn e m h s ib ru fe R y g re n e la n o ita re p Oe s u re ta w la n o ita re p Oe s u n o itc u rts n o c -e Dn o itilo m e d tro p s n a rT g n is s e c o rp e ts a W la s o p s iD -e s u e R-y re v o c e R-g n ilc y c e Rla itn e to p
A1 A2 A3 A4 A5 B1 B2 B3 B4 B5 B6 B7 C1 C2 C3 C4 D
X X X MND X X X MNR MNR MNR X MND X X X X X
RESULTS OF THE LCA - ENVIRONMENTAL IMPACT according to EN 15804+A2: 1 m2 VELUX soft shutter SSS of the size
MK06 = area of 0.919 m2 (0.78 m * 1.178 m)
Parameter Unit A1-A3 A5 B1 B2 B6 C1 C2 C3 C4 D
GWP-total kg CO 2 eq 1.37E+02 3.98E+00 0 8.28E+00 0 0 1.62E-01 1.62E+00 4.07E+00 -1.18E+02
GWP-fossil kg CO 2 eq 1.4E+02 1.32E+00 0 8.23E+00 0 0 1.62E-01 1.33E+00 4.07E+00 -1.17E+02
GWP-
biogenic kg CO 2 eq -2.96E+00 2.66E+00 0 0 0 0 0 2.98E-01 0 0
GWP-luluc kg CO 2 eq 3.76E-01 3.38E-05 0 4.96E-02 0 0 6.61E-05 3.7E-04 9.97E-05 -4.33E-01
ODP kg CFC11 eq 8.46E-06 1.89E-08 0 7.88E-07 0 0 3.81E-08 2.3E-08 3.47E-08 -3.97E-06
AP mol H+ eq 1.01E+00 5.73E-04 0 1.87E-01 0 0 9.21E-04 1.51E-03 1.3E-03 -7.53E-01
EP-
kg P eq 5.81E-03 6.73E-07 0 4.45E-04 0 0 1.19E-06 3.94E-05 3.09E-06 -4.42E-03
freshwater
EP-marine kg N eq 1.45E-01 2.2E-04 0 9.87E-03 0 0 3.31E-04 5.21E-04 5.55E-04 -1.12E-01
EP-terrestrial mol N eq 1.54E+00 2.44E-03 0 1.02E-01 0 0 3.64E-03 5.73E-03 5.86E-03 -1.23E+00
kg NMVOC
POCP 4.96E-01 6.84E-04 0 4.03E-02 0 0 1.04E-03 1.5E-03 1.44E-03 -3.64E-01
eq
ADPE kg Sb eq 3.07E-03 2.82E-07 0 9.62E-04 0 0 5.44E-07 6.28E-07 8.27E-07 1.01E-03
ADPF MJ 1.61E+03 1.23E+00 0 9.23E+01 0 0 2.5E+00 4.57E+00 1.06E+00 -1.07E+03
m3 world eq
WDP 5.58E+01 5.87E-03 0 6.66E+00 0 0 8.21E-03 7.09E-02 6.76E-02 -1.57E+01
deprived
GWP = Global warming potential; ODP = Depletion potential of the stratospheric ozone layer; AP = Acidification potential of land and water; EP =
Eutrophication potential; POCP = Formation potential of tropospheric ozone photochemical oxidants; ADPE = Abiotic depletion potential for non-fossil
resources; ADPF = Abiotic depletion potential for fossil resources; WDP = Water (user) deprivation potential)
RESULTS OF THE LCA - INDICATORS TO DESCRIBE RESOURCE USE according to EN 15804+A2: 1 m2 VELUX soft shutter
SSS of the size MK06 = area of 0.919 m2 (0.78 m * 1.178 m)
Parameter Unit A1-A3 A5 B1 B2 B6 C1 C2 C3 C4 D
PERE MJ 1.92E+02 1.98E-02 0 2.46E+01 1.33E+03 0 3.53E-02 5.48E-01 9.04E-02 -1.42E+02
PERM MJ 3.44E+01 -3.06E+01 0 0 0 0 0 -3.84E+00 0 0
PERT MJ 2.27E+02 1.98E-02 0 2.46E+01 1.33E+03 0 3.53E-02 -3.29E+00 9.04E-02 -1.42E+02
PENRE MJ 1.53E+03 2.04E+01 0 9.11E+01 0 0 2.5E+00 4.6E-06 5.74E+01 -1.07E+03
PENRM MJ 7.55E+01 -1.91E+01 0 0 0 0 0 0 -5.64E+01 0
PENRT MJ 1.61E+03 1.23E+00 0 9.11E+01 0 0 2.5E+00 4.6E-06 1.06E+00 -1.07E+03
SM kg 5.65E-01 0 0 3.41E-02 0 0 0 0 0 8.5E+00
RSF MJ 0 0 0 0 0 0 0 0 0 0
NRSF MJ 0 0 0 0 0 0 0 0 0 0
FW m3 2.33E+00 2.2E-04 0 1.13E+00 0 0 4.14E-04 7.62E-04 9.28E-04 1.1E+00
PERE = Use of renewable primary energy excluding renewable primary energy resources used as raw materials; PERM = Use of renewable primary
energy resources used as raw materials; PERT = Total use of renewable primary energy resources; PENRE = Use of non-renewable primary energy
excluding non-renewable primary energy resources used as raw materials; PENRM = Use of non-renewable primary energy resources used as raw
materials; PENRT = Total use of non-renewable primary energy resources; SM = Use of secondary material; RSF = Use of renewable secondary fuels;
NRSF = Use of non-renewable secondary fuels; FW = Use of net fresh water
RESULTS OF THE LCA – WASTE CATEGORIES AND OUTPUT FLOWS according to EN 15804+A2:
1 m2 VELUX soft shutter SSS of the size MK06 = area of 0.919 m2 (0.78 m * 1.178 m)
Parameter Unit A1-A3 A5 B1 B2 B6 C1 C2 C3 C4 D
HWD kg 3.96E-02 3.34E-06 0 1.16E-03 0 0 6.37E-06 4.6E-06 3.56E-06 1.54E-02
NHWD kg 3.46E+01 9.32E-02 0 3.73E+00 0 0 1.68E-01 5.14E-01 2.09E-01 -2.83E+01
6 Environmental Product Declaration - VELUX A/S - VELUX soft shutter - solar-powered
RWD kg 7.5E-03 1.73E-05 0 6.3E-04 0 0 3.61E-05 4.06E-05 7.01E-06 -3.33E-03
CRU kg 0 0 0 0 0 0 0 0 0 0
MFR kg 8.38E-01 1.81E+00 0 8.21E-01 0 0 0 7.54E+00 0 0
MER kg 0 0 0 0 0 0 0 0 0 0
EEE MJ 1.64E-01 2.49E+00 0 5.05E-01 0 0 0 0 7.33E+00 0
EET MJ 3.23E-01 4.89E+00 0 9.94E-01 0 0 0 0 1.44E+01 0
HWD = Hazardous waste disposed; NHWD = Non-hazardous waste disposed; RWD = Radioactive waste disposed; CRU = Components for re-use;
MFR = Materials for recycling; MER = Materials for energy recovery; EEE = Exported electrical energy; EET = Exported thermal energy
RESULTS OF THE LCA – additional impact categories according to EN 15804+A2-optional:
1 m2 VELUX soft shutter SSS of the size MK06 = area of 0.919 m2 (0.78 m * 1.178 m)
Parameter Unit A1-A3 A5 B1 B2 B6 C1 C2 C3 C4 D
Disease
PM 9.62E-06 7.96E-09 0 6.15E-07 0 0 1.46E-08 1.97E-08 7.51E-09 -9E-06
incidence
IR kBq U235 eq 3.97E+00 5.26E-03 0 4.3E-01 0 0 1.09E-02 1.59E-02 3.7E-03 -1.24E+00
ETP-fw CTUe 4.08E+03 1.23E+00 0 5.41E+02 0 0 1.98E+00 8.65E+00 1.48E+01 -2.38E+03
HTP-c CTUh 2.1E-07 1.88E-10 0 3.33E-08 0 0 7.9E-11 1.52E-10 7.17E-10 -1.3E-07
HTP-nc CTUh 4.15E-06 2.21E-09 0 6.18E-07 0 0 2.28E-09 1.57E-08 7.54E-09 -2.05E-06
SQP SQP 4.91E+02 1.03E+00 0 4.06E+01 0 0 2.13E+00 8.28E-01 3.61E-01 -1.54E+02
PM = Potential incidence of disease due to PM emissions; IR = Potential Human exposure efficiency relative to U235; ETP-fw = Potential comparative
Toxic Unit for ecosystems; HTP-c = Potential comparative Toxic Unit for humans (cancerogenic); HTP-nc = Potential comparative Toxic Unit for humans
(not cancerogenic); SQP = Potential soil quality index
Disclaimer 1 – for the indicator 'Potential Human exposure efficiency relative to U235'.This impact category deals mainly with the
eventual impact of low dose ionizing radiation on human health of the nuclear fuel cycle. It does not consider effects due to possible
nuclear accidents, occupational exposure or radioactive waste disposal in underground facilities. Potential ionizing radiation from the
soil, radon and from some construction materials is also not measured by this indicator.
Disclaimer 2 – for the indicators 'abiotic depletion potential for non-fossil resources', 'abiotic depletion potential for fossil resources',
'water (user) deprivation potential, deprivation-weighted water consumption', 'potential comparative toxic unit for ecosystems', 'potential
comparative toxic unit for humans – cancerogenic', 'Potential comparative toxic unit for humans - not cancerogenic', 'potential soil
quality index'. The results of this environmental impact indicator shall be used with care as the uncertainties on these results are high
as there is limited experience with the indicator.
6. LCA: Interpretation
Figure 1 illustrates the relative contributions of the different
modules along the life cycle of the declared products.
Figure 1: Relative environmental impacts of the different insignificant (around 4 %) with exception of the ADP elements,
life cycle stages for the shutter SSS with solar-powered where copper and other rather rare metals add to this impact
motor category (module B2).
Benefits and burdens beyond the system boundary (module D)
The largest part of environmental impacts – between 85 % and are in the order of 50 % to 80 % of the impacts over the product
rather 90 % - is caused during production (modules A1-A3) of life cycle (modules A1-C4). The net positive impact ('load') of
the shutter and its motor. Operational energy use is insignificant the ADPelements is related to copper input as the copper
due to the use of solar power (the PV-cell, batteries etc. are cathode for the remelting of recycled aluminium.[1] The use of
taken into account in modules A5. The replacement of the renewable primary energy is mainly caused by the share of
motor – the disposal of the obsolete motor and the production renewable energy in the electricity mix and the use of solar
of and installation of its replacement – is comparably power as operational energy input, thus the production stage
7 Environmental Product Declaration - VELUX A/S - VELUX soft shutter - solar-powered
and the use of operational energy are the main drivers of this are mainly caused by the European electricity mix used during
impact category; for the use of non-renewable primary energy, the use phase.
the production phase is thus the most impacting life cycle
stage. Except for the ADPelements (where the contributions are 45 %
Material use of primary energy is negligible and related to of the impacts of the soft shutter itself), the contributions of the
plastic parts of the product and packaging material. The motor as compared to the base unit are small (around 10 % to
material use of primary energy is transferred to its energy use 20 %).
when the materials containing primary energy are incinerated
with energy recovery. [1] Benefits resulting from the recycling of plastics as well as
Non-hazardous waste as the quantitatively most relevant waste from the recycling of the electronic parts are disregarded due to
flows is mainly caused during maintenance due to the the lack of data on the recycling processes and related to the
replacement of the motor; hazardous and radio-active wastes detailed composition of the electronic parts.
7. Requisite evidence
8 Environmental Product Declaration - VELUX A/S - VELUX soft shutter - solar-powered
VOC testing is not required for products without contact to indoor air.
8. References
PProduct category rules of IBU EN 13659
EN 13659:2015, Shutters and external venetian blinds -
IBU (2021) Performance requirements including safety
IBU (2021): General Instructions for the EPD Programme of the
Institut Bauen & Umwelt e.V. (General Instructions for the IBU EN 16485
EPD Programme). Version 2.0, Institut Bauen & Umwelt, Berlin DIN EN 16485:2014-07, Round and sawn timber -
Environmental Product Declarations - Product category rules
IBU (2017) for wood and wood-based products for use in construction;
IBU (2017): PCR Teil A: PCR Part A: Calculation rules for the German version EN 16485:2014.
life cycle assessment and requirements for the project report.
Version 1.8., Institut Bauen & Umwelt, Berlin. ECHA-List
The Candidate List of substances of very high concern,
IBU (2019) available via https://echa.europa.eu/nl/-/four-newsubstances-
IBU (2019): PCR Part B: Requirements on the EPD for sun added-to-the-candidate-list.
protection systems. Version 2019/07, Institut Bauen & Umwelt,
Berlin. Regulation on biocidal products
REGULATION (EU) No 528/2012 OF THE EUROPEAN
Standards and legal documents PARLIAMENT AND OF THE COUNCIL of 22 May 2012
concerning the making available on the market and use of
EN 15804 biocidal products.
DIN EN 15804+A2:2019, Sustainability of construction works -
Environmental product declarations - Core rules for the product Regulation (EU) Nr. 305/2011(CPR)
category construction products. REGULATION (EU) No 305/2011 OF THE EUROPEAN
PARLIAMENT AND OF THE COUNCIL of 9 March 2011 laying
ISO 14025 down harmonised conditions for the marketing of construction
DIN EN ISO 14025:2006-07, Environmental labels and products and repealing Council Directive 89/106/EEC
declarations - Type III Environmental declarations - Principles
and procedures. COUNCIL REGULATION (EU) No 333/2011
COUNCIL REGULATION (EU) No 333/2011 of 31 March 2011
ISO 14044 establishing criteria determining when certain types of scrap
DIN EN ISO 14044:2006-07, Environmental management - Life metal cease to be waste under Directive 2008/98/EC of the
cycle assessment - Requirements and guidance (ISO European Parliament and of the Council.
14044:2006); German and English versions EN ISO
14044:2006. European Waste List (Waste index)
http://www.gesetze-im-internet.de/avv/anlage.htm
ISO 9001
DIN EN ISO 9001:2015, Quality management systems - Additional references
Requirements.
Weidema et al. (2013)
ISO 14001 Weidema, B., C. Bauer, R. Hischier, C. Mutel, T. Nemecek, J.
DIN EN ISO 14001:2015: Environmental management Reinhard, C.O. Vadenbo, G. Wernet (2013): Overview and
systems - Requirements with guidance for use. methodology, Data quality guideline for the ecoinvent database
version 3. ecoinvent report no. 1 (v3), St. Gallen, Schweiz.
ISO 45001
ISO 45001:2018-03, Occupational health and safety ecoinvent 3.8
management systems - Requirements with guidance for use. ecoinvent 3.8, LCA database, 12/2021. Ecoinvent centre,
Zürich.
9 Environmental Product Declaration - VELUX A/S - VELUX soft shutter - solar-powered
Publisher
Institut Bauen und Umwelt e.V. +49 (0)30 3087748- 0
Hegelplatz 1 info@ibu-epd.com
10117 Berlin www.ibu-epd.com
Germany
Programme holder
Institut Bauen und Umwelt e.V. +49 (0)30 3087748- 0
Hegelplatz 1 info@ibu-epd.com
10117 Berlin www.ibu-epd.com
Germany
Author of the Life Cycle Assessment
Dr. Frank Werner - Umwelt & Entwicklung + 41 (0)44 241 39 06
Kammelenbergstrasse 30 frank@frankwerner.ch
9011 St. Gallen http://www.frankwerner.ch/
Switzerland
Owner of the Declaration
VELUX Group +4545164726
Ådalsvej 99 jakob.roerbech@velux.com
2970 Hørsholm www.velux.com
Denmark
10 Environmental Product Declaration - VELUX A/S - VELUX soft shutter - solar-powered
