Environmental product declaration
in accordance with ISO 14025 and EN 15804+A2
VEX1030RS
Owner of the declaration: Program operator:
EXHAUSTO AS The Norwegian EPD Foundation
Product: Declaration number:
VEX1030RS
NEPD-8571-8232-EN
Declared unit:
Registration number:
1 pcs
NEPD-8571-8232-EN
This declaration is based on Product Category Rules:
CEN Standard EN 15804:2012+A2:2019 serves as core Issue date: 19.12.2024
PCR Valid to: 19.12.2029
The Norwegian EPD Foundation NPCR 030:2021 Part B for ventilation components
EPD software:
LCAno EPD generator ID: 716263
1 / 15
General information
Product Owner of the declaration:
VEX1030RS EXHAUSTO AS
Contact person: Lars R. Reinemo
Phone: +47 63 87 07 70
e-mail: lrr@exhausto.no
Program operator: Manufacturer:
The Norwegian EPD Foundation EXHAUSTO A/S
Post Box 5250 Majorstuen, 0303 Oslo, Norway
Phone: +47 977 22 020
web: www.epd-norge.no
Declaration number: Place of production:
EXHAUSTO A/S
NEPD-8571-8232-EN
Odensevej 76
DK-5550 Langeskov, Denmark
This declaration is based on Product Category Rules: Management system:
CEN Standard EN 15804:2012+A2:2019 serves as core PCR ISO 9001
NPCR 030:2021 Part B for ventilation components
Statement of liability: Organisation no:
The owner of the declaration shall be liable for the underlying 812 701 002
information and evidence. EPD Norway shall not be liable with respect
to manufacturer information, life cycle assessment data and
evidences.​
Declared unit: Issue date:
1 pcs VEX1030RS 19.12.2024
Declared unit with option: Valid to:
A1-A3,A4,A5,B1,B2,B3,B4,B5,B6,B7,C1,C2,C3,C4,D 19.12.2029
Year of study:
2024
Functional unit: Comparability:
1 ventilation unit EPD of construction products may not be comparable if they not
comply with EN 15804 and seen in a building context.
General information on verification of EPD from EPD tools: Development and verification of EPD:
Independent verification of data, other environmental information The declaration is created using EPD tool lca.tools ver EPD2022.03,
and the declaration according to ISO 14025:2010, § 8.1.3 and § 8.1.4. developed by LCA.no. The EPD tool is integrated in the company's
Verification of each EPD is made according to EPD-Norway’s management system and has been approved by EPD Norway.
guidelines for verification and approval requiring that tools are i) NEPDT46 VKEs EPD-generator
integrated into the company's environmental management system, ii)
the procedures for use of the EPD tool are approved by EPD-Norway, Developer of EPD: Rasmus Runge Bechsgaard
and iii) the process is reviewed annually by an independent third
Reviewer of company-specific input data and EPD:​ Henning Grønbæk
party verifier. See Appendix G of EPD-Norway's General Programme
Instructions for further information on EPD tools
Verification of EPD tool: Approved:
Independent third party verification of the EPD tool, background data
and test-EPD in accordance with EPDNorway's procedures and
guidelines for verification and approval of EPD tools.
Third party verifier:
Alexander Borg, Asplan Viak AS
(no signature required)
2 / 15
Product
Product description:
VEX1030RS, compact air handling unit with rotary heat exchanger
Product specification
Materials kg %
Adhesive 0,75 0,22
Electronic - Unspecified 1,50 0,43
Filter, mineral based 0,80 0,23
Glass fibre reinforced plastic,
7,55 2,17
polyamide
Insulation, Mineral based 33,00 9,46
Motor 22,65 6,50
Plastic - Acrylonitrile butadiene
0,73 0,21
styrene (ABS)
Plastic - Polyamide 0,59 0,17
Rubber, synthetic 2,12 0,61
Metal - Aluminium 59,00 16,92
Metal - Stainless steel 10,04 2,88
Metal - Steel 204,45 58,64
Other 5,00 1,43
Plastic - Polycarbonate (PC) 0,50 0,14
Total 348,68 100,00
Technical data:
See our calculation tool: EXselectPRO
Market:
Europe.
Reference service life, product
25 years.
Reference service life, building or construction works
50 years.
LCA: Calculation rules
Declared unit:
1 pcs VEX1030RS
Cut-off criteria:
All major raw materials and all the essential energy is included. The production processes for raw materials and energy flows with very small
amounts (less than 1%) are not included. These cut-off criteria do not​ apply for hazardous materials and substances.
Allocation:
The allocation is made in accordance with the provisions of EN 15804. Energy, water and waste production in-house is allocated equally among all
products through mass allocation. Effects of primary production of recycled materials is allocated to the main product in which the material was
used. The recycling process and transportation of the material is allocated to this analysis. The allocation is made in accordance with the provisions
of EN 15804. Energy, water and waste production in-house is allocated equally among all
products through mass allocation. Effects of primary production of recycled materials is allocated to the main product in which the material was
used. The recycling process and transportation of the material is allocated to this analysis.
Data quality:
Specific data for the product composition are provided by the manufacturer. The data represent the production of the declared product and were
collected for EPD development in the year of study. Background data is based on EPDs according to EN 15804 and different LCA databases. The
data quality of the raw materials in A1 is presented in the table below.
3 / 15
Materials Source Data quality Year
Adhesive ecoinvent 3.6 Database 2019
Electronic - Unspecified ecoinvent 3.6 Database 2019
Filter, mineral based ecoinvent 3.6 Database 2019
Glass fibre reinforced plastic, polyamide Modified ecoinvent 3.6 Database 2019
Insulation, Mineral based ecoinvent 3.6 Database 2019
Metal - Aluminium Modified ecoinvent 3.6 Database 2019
Metal - Stainless steel ecoinvent 3.6 Database 2019
Metal - Steel ecoinvent 3.6 Database 2019
Motor Modified ecoinvent 3.6 Database 2019
Supplier data +
Other Material composition + ecoinvent 3.6 2019
database
Plastic - Acrylonitrile butadiene styrene (ABS) ecoinvent 3.6 Database 2019
Plastic - Polyamide ecoinvent 3.6 Database 2019
Plastic - Polycarbonate (PC) ecoinvent 3.6 Database 2019
Rubber, synthetic ecoinvent 3.6 Database 2019
4 / 15
System boundaries (X=included, MND=module not declared, MNR=module not relevant)
Construction Beyond the system
Product stage Use stage End of life stage
installation stage boundaries
A1 A2 A3 A4 A5 B1 B2 B3 B4 B5 B6 B7 C1 C2 C3 C4 D
X X X X X X X X X X X X X X X X X
System boundary:
waR slairetam tropsnarT gnirutcafunaM tropsnarT ylbmessA e​sU ecnanetniaM riapeR tnemecalpeR tnemhsibrufeR lanoitarepO ygrene esu lanoitarepO esu retaw -eD noitcurtsnoc noitilomed tropsnarT etsaW gnissecorp lasopsiD -yrevoceR-esueR laitnetop-gnilcyceR
5 / 15
This EPD is based on a cradle-to-gate with options, modules C1-C3 and module D cf. EN 15804 + A2, in which 100%-weight of the products have
been accounted for.
The general rules for the exclusion of inputs and outputs follows the requirements in EN 15804, 6.3.5, where the total of neglected input flows per
module shall be a maximum of 5 % of energy usage and mass and 1 % of energy usage and mass for unit processes.
Excluded processes:
- Use of electric screwdrivers during installation (module A5), and disassembly (module C1)
Product stage (A1-A3) includes:
A1 – Extraction and processing of raw materials
A2 – Transport to the production site
A3 – Manufacturing processes
A1-3: The product stage includes all the raw materials, products and energy, transport to the production site, packaging and waste processing up
to the ”end-of-waste” state or final disposal. The LCA results are declared in aggregated form for the product stage, which means, that the sub-
modules A1, A2 and A3 are declared as one module A1-A3.
Construction process stage (A4-A5) includes:
A4: Transportation to the building site, is assumed to be an average of 300km.
A5: Treatment of the plastic folio used as packaging material.
Use stage (B1-B7) includes:
B1: This module has no activity.
B2: To maintain the performance of the ventilation unit and ensure a continuous supply of fresh ventilated air continuously throughout the
lifespan, it is necessary to replace the ventilation filters. The production of new filters and the waste treatment of the replaced filters are included in
B2. There is calculated with one filter replacement per year, to best fit the market trends. (However, EXHAUSTO recommends replacement of the
filters twice a year to maintain optimal IAQ) It is important to note that B2 is modelled for one year and does not represent the lifespan of 25
years.
B3-B5: No repair, replacement, or refurbishment due to damage is expected within the reference service life of 25 years.
B6: No specification regarding use is described in EN 50693:2019. Therefore, the Ecodesign Directive (COMMISSION REGULATION (EU) No
1253/2014 of 7 July 2014 implementing Directive 2009/125/EC of the European Parliament and of the Council with regard to Ecodesign
requirements for ventilation units) is used to determine the reference capacity and thus the energy use of the ventilation unit. The Ecodesign
requirements specify a reference flow rate set at 70% of the maximum flow rate. The annual operating hours are set to 8,760 hours per year as a
conservative approach which is in accordance with the default value that is used in the Ecodesign directive to calculate the SEC (specific energy
consumption).
B6 is modelled for 1 year.
B7: This module has no activity.
End of Life (C1-C4) includes:
For the end-of-life scenario, a collection rate of 100% is assumed.
C1: No impacts from dismantling have been included in this module it is done manually.
C2: Transportation to local recycling is assumed to be 200km.
C3: The average waste treatment for the different materials has been utilised.
C4: The average landfilling for the different materials has been utilised.
Re-use, recovery, and recycling potential (D) includes:
D: Potential benefits from recovery and recycling of materials from the product are calculated. The materials are either used as secondary material
in a new product system, thus substituting virgin material, or incinerated with energy recovery.
6 / 15
Additional technical information:
7 / 15
LCA: Scenarios and additional technical information
The following information describe the scenarios in the different modules of the EPD.
Capacity utilisation Value
Transport from production place to user (A4) Distance (km) Fuel/Energy Consumption Unit
(incl. return) % (Liter/tonne)
Truck, 16-32 tonnes, EURO 6 (km) 36,7 % 300 0,043 l/tkm 12,90
Assembly (A5) Unit Value
Waste, plastic, mixture, to average treatment - A5,
kg/DU 0,12
inkl. transp. (kg)
Maintenance (B2) Unit Value
Filter component - ABS frame (kg) - Europe kg 0,73
Filter component - Glass fibre (kg) - Europe kg 0,80
Filter component - Glue, Polymeric mastic (kg) -
kg 0,48
Europe
Filter component - Hot glue (kg) - Europe kg 0,27
Operational energy (B6) Unit Value
Electricity, Denmark (kWh) kWh 18148,00
De-construction demolition (C1) Unit Value
Demolition of building per kg of ventilation
kg 348,68
product (kg)
Capacity utilisation Value
Transport to waste processing (C2) Distance (km) Fuel/Energy Consumption Unit
(incl. return) % (Liter/tonne)
Truck, 16-32 tonnes, EURO 6 (km) 36,7 % 200 0,043 l/tkm 8,60
Waste processing (C3) Unit Value
Materials to recycling (kg) kg 270,76
Waste treatment per kg wire plastic, municipal
kg 1,17
incineration - C3 - RoW
Waste treatment per kg Electronics scrap, Control
kg 1,50
units, incineration (kg)
Waste treatment per kg Plastics, from incineration
kg 4,32
(kg)
Waste treatment per kg Hazardous waste,
kg 0,75
incineration (kg)
Waste treatment per kg plastic, industrial
electronics, municipal incineration with fly ash kg 0,36
extraction (kg)
Waste treatment per kg Bulk iron waste, excluding
kg 22,65
reinforcement, sorting plant (kg)
Waste treatment per kg Rubber, municipal
kg 2,12
incineration with fly ash extraction (kg)
Disposal (C4) Unit Value
Landfilling of ashes from incineration per kg wire
kg 0,17
plastic, from municipal incineration - C4 - RoW
Waste treatment per kg Copper slag, to landfill,
kg 0,63
residual material landfill (kg) - GLO
Waste, plastic, mixture, to landfill (kg) kg 5,85
Landfilling of ashes from incineration of
Electronics scrap, Control units, process of ashes kg 1,05
and residues (kg)
Landfilling of ashes from incineration of Plastics,
kg 0,10
process per kg ashes and residues (kg)
Landfilling of ashes from incineration per kg
kg 0,14
Hazardous waste, from incineration (kg)
Waste, mineral wool, to landfil (kg) kg 33,80
Landfilling of ashes from incineration per kg
plastic, industrial electronics, From municipal kg 0,02
incineration with fly ash extraction (kg)
Waste, scrap steel, to landfill (kg) kg 23,15
Waste, aluminium, to landfill (kg) kg 4,27
Landfilling of ashes from incineration of Rubber,
kg 0,11
municipal incineration with fly ash extraction (kg)
Benefits and loads beyond the system
Unit Value
boundaries (D)
Substitution of electricity, in Norway (MJ) MJ 4,95
Substitution of thermal energy, district heating, in
MJ 74,95
Norway (MJ)
Substitution of primary copper with net scrap (kg) kg 3,32
Substitution of primary steel with net scrap (kg) kg 169,15
Substitution of primary aluminium with net scrap
kg 54,62
(kg)
8 / 15
9 / 15
LCA: Results
The LCA results are presented below for the declared unit defined on page 2 of the EPD document.
Environmental impact
Indicator Unit A1-A3 A4 A5 B1 B2 B3 B4
GWP-total kg CO2 -eq 2,51E+03 1,71E+01 9,51E-03 0 1,48E+01 0 0
GWP-fossil kg CO2 -eq 2,50E+03 1,71E+01 9,50E-03 0 1,48E+01 0 0
GWP-biogenic kg CO2 -eq 8,71E+00 7,07E-03 1,31E-06 0 4,25E-02 0 0
GWP-luluc kg CO2 -eq 9,82E-01 6,08E-03 7,29E-07 0 6,18E-03 0 0
ODP kg CFC11 -eq 1,02E-04 3,87E-06 5,71E-10 0 1,46E-06 0 0
AP mol H+ -eq 1,96E+01 4,91E-02 1,17E-05 0 5,88E-02 0 0
EP-FreshWater kg P -eq 1,04E-01 1,37E-04 1,96E-08 0 3,54E-04 0 0
EP-Marine kg N -eq 2,73E+00 9,72E-03 1,07E-05 0 1,22E-02 0 0
EP-Terrestial mol N -eq 4,32E+01 1,09E-01 4,20E-05 0 1,33E-01 0 0
POCP kg NMVOC -eq 9,51E+00 4,16E-02 1,38E-05 0 4,51E-02 0 0
ADP-minerals&metals1 kg Sb-eq 5,17E-01 4,72E-04 5,06E-08 0 4,37E-04 0 0
ADP-fossil1 MJ 2,43E+04 2,58E+02 3,92E-02 0 2,19E+02 0 0
WDP1 m3 3,41E+04 2,50E+02 1,39E-01 0 4,96E+02 0 0
Indicator Unit B5 B6 B7 C1 C2 C3 C4 D
GWP-total kg CO2 -eq 0 6,14E+03 0 4,60E-01 1,14E+01 2,37E+01 1,26E+00 -6,91E+02
GWP-fossil kg CO2 -eq 0 6,07E+03 0 4,60E-01 1,14E+01 2,37E+01 1,26E+00 -6,79E+02
GWP-biogenic kg CO2 -eq 0 6,29E+01 0 8,62E-05 4,71E-03 8,48E-03 7,54E-04 -2,37E+00
GWP-luluc kg CO2 -eq 0 8,17E+00 0 3,62E-05 4,05E-03 8,26E-04 1,77E-04 -9,32E+00
ODP kg CFC11 -eq 0 2,06E-04 0 9,94E-08 2,58E-06 3,31E-07 1,72E-07 -3,17E-02
AP mol H+ -eq 0 2,43E+01 0 4,81E-03 3,27E-02 6,86E-03 4,20E-03 -5,55E+00
EP-FreshWater kg P -eq 0 4,97E-01 0 1,67E-06 9,10E-05 5,56E-05 7,46E-06 -3,92E-02
EP-Marine kg N -eq 0 4,09E+00 0 2,12E-03 6,48E-03 2,10E-03 2,14E-03 -6,62E-01
EP-Terrestial mol N -eq 0 5,84E+01 0 2,33E-02 7,25E-02 2,23E-02 1,60E-02 -7,38E+00
POCP kg NMVOC -eq 0 1,25E+01 0 6,40E-03 2,78E-02 5,75E-03 4,73E-03 -2,70E+00
ADP-minerals&metals1 kg Sb-eq 0 5,40E-02 0 7,05E-07 3,15E-04 1,47E-05 7,01E-06 -9,93E-03
ADP-fossil1 MJ 0 7,86E+04 0 6,33E+00 1,72E+02 1,27E+01 1,23E+01 -7,81E+03
WDP1 m3 0 1,22E+06 0 1,34E+00 1,67E+02 7,88E+01 6,69E+01 -2,68E+05
GWP-total = Global Warming Potential total; GWP-fossil = Global Warming Potential fossil fuels; GWP-biogenic = Global Warming Potential biogenic; GWP-luluc =
Global Warming Potential land use and land use change; ODP = Depletion potential of the stratospheric ozone layer; AP = Acidification potential, Accumulated
Exceedance; EP-freshwater = Eutrophication potential, fraction of nutrients reaching freshwater end compartment: EP-marine = Eutrophication potential, fraction of
nutrients reaching marine end compartment; EP-terrestrial = Eutrophication potential, Accumulated Exceedance; POCP = Formation potential of tropospheric ozone;
ADP-minerals&metals = Abiotic depletion potential for non-fossil resources; ADP-fossil = Abiotic depletion for fossil resources potential; WDP = Water (user)
deprivation potential, deprivation-weighted water consumption
"Reading example: 9,0 E-03 = 9,0*10-3 = 0,009"
*INA Indicator Not Assessed
1. The results of this environmental impact indicator shall be used with care as the uncertainties on these results are high or as there is limited experienced with the
indicator
Remarks to environmental impacts
10 / 15
Additional environmental impact indicators
Indicator Unit A1-A3 A4 A5 B1 B2 B3 B4
PM Disease incidence 2,24E-04 1,05E-06 2,11E-10 0 5,13E-07 0 0
IRP2 kgBq U235 -eq 4,08E+01 1,13E+00 1,77E-04 0 5,18E-01 0 0
ETP-fw1 CTUe 1,03E+05 1,92E+02 3,74E-02 0 2,22E+02 0 0
HTP-c1 CTUh 7,62E-06 0,00E+00 1,00E-12 0 1,11E-08 0 0
HTP-nc1 CTUh 9,09E-05 2,09E-07 3,50E-11 0 2,37E-07 0 0
SQP1 dimensionless 7,83E+03 1,81E+02 6,84E-02 0 4,62E+01 0 0
Indicator Unit B5 B6 B7 C1 C2 C3 C4 D
PM Disease incidence 0 1,19E-04 0 1,27E-07 6,97E-07 6,26E-08 7,67E-08 -5,22E-05
IRP2 kgBq U235 -eq 0 3,85E+02 0 2,71E-02 7,53E-01 5,70E-02 5,64E-02 -2,63E+01
ETP-fw1 CTUe 0 1,40E+05 0 3,46E+00 1,28E+02 1,65E+02 2,66E+03 -3,00E+04
HTP-c1 CTUh 0 2,76E-06 0 0,00E+00 0,00E+00 3,01E-09 1,50E-08 -2,30E-06
HTP-nc1 CTUh 0 9,16E-05 0 3,14E-09 1,39E-07 7,70E-08 1,01E-06 -9,70E-06
SQP1 dimensionless 0 1,29E+05 0 8,03E-01 1,20E+02 4,55E+00 3,31E+01 -3,67E+02
PM = Particulate Matter emissions; IRP = Ionizing radiation – human health; ETP-fw = Eco toxicity – freshwater; HTP-c = Human toxicity – cancer effects; HTP-nc =
Human toxicity – non cancer effects; SQP = Potential Soil Quality Index (dimensionless)
"Reading example: 9,0 E-03 = 9,0*10-3 = 0,009"
*INA Indicator Not Assessed
1. The results of this environmental impact indicator shall be used with care as the uncertainties on these results are high or as there is limited experienced with the
indicator
2. This impact category deals mainly with the eventual impact of low dose ionizing radiation on human health of the nuclear fuel cycle. It does not consider effects due
to possible nuclear accidents, occupational exposure nor due to radioactive waste disposal in underground facilities. Potential ionizing radiation from the soil, from
radon and from some construction materials is also not measured by this indicator.
11 / 15
Resource use
Indicator Unit A1-A3 A4 A5 B1 B2 B3 B4
PERE MJ 2,14E+03 3,70E+00 9,90E-04 0 9,35E+00 0 0
PERM MJ 0,00E+00 0,00E+00 0,00E+00 0 0,00E+00 0 0
PERT MJ 2,14E+03 3,70E+00 9,90E-04 0 9,35E+00 0 0
PENRE MJ 2,39E+04 2,58E+02 3,92E-02 0 1,68E+02 0 0
PENRM MJ 4,22E+02 0,00E+00 0,00E+00 0 0,00E+00 0 0
PENRT MJ 2,43E+04 2,58E+02 3,92E-02 0 1,68E+02 0 0
SM kg 2,84E+01 0,00E+00 0,00E+00 0 0,00E+00 0 0
RSF MJ 2,90E+01 1,32E-01 2,60E-05 0 5,01E-01 0 0
NRSF MJ 4,14E+02 4,73E-01 6,80E-05 0 2,37E-01 0 0
FW m3 1,31E+01 2,76E-02 2,07E-05 0 1,22E-01 0 0
Indicator Unit B5 B6 B7 C1 C2 C3 C4 D
PERE MJ 0 6,76E+04 0 3,42E-02 2,47E+00 1,89E+00 4,48E-01 -2,43E+03
PERM MJ 0 0,00E+00 0 0,00E+00 0,00E+00 0,00E+00 0,00E+00 0,00E+00
PERT MJ 0 6,76E+04 0 3,42E-02 2,47E+00 1,89E+00 4,48E-01 -2,43E+03
PENRE MJ 0 7,87E+04 0 6,33E+00 1,72E+02 1,27E+01 1,23E+01 -7,81E+03
PENRM MJ 0 0,00E+00 0 0,00E+00 0,00E+00 0,00E+00 0,00E+00 0,00E+00
PENRT MJ 0 7,87E+04 0 6,33E+00 1,72E+02 1,27E+01 1,23E+01 -7,81E+03
SM kg 0 0,00E+00 0 3,11E-03 0,00E+00 2,50E-04 1,26E-04 2,32E+00
RSF MJ 0 2,54E+03 0 8,42E-04 8,82E-02 4,09E-02 9,52E-03 6,02E+00
NRSF MJ 0 1,34E+01 0 1,24E-02 3,15E-01 -6,72E-04 2,59E-02 1,97E+02
FW m3 0 2,51E+02 0 3,26E-04 1,84E-02 9,01E-02 1,64E-02 -1,28E+01
PERE = Use of renewable primary energy excluding renewable primary energy resources used as raw materials; PERM = Use of renewable primary energy resources used
as raw materials; PERT = Total use of renewable primary energy resources; PENRE = Use of non renewable primary energy excluding non-renewable primary energy
resources used as raw materials; PENRM = Use of non renewable primary energy resources used as raw materials; PENRT = Total use of non renewable primary energy
resources; SM = Use of secondary materials; RSF = Use of renewable secondary fuels; NRSF = Use of non-renewable secondary fuels; FW = Net use of fresh water
"Reading example: 9,0 E-03 = 9,0*10-3 = 0,009"
*INA Indicator Not Assessed
12 / 15
End of life - Waste
Indicator Unit A1-A3 A4 A5 B1 B2 B3 B4
HWD kg 1,54E+01 1,33E-02 0,00E+00 0 4,43E-02 0 0
NHWD kg 6,31E+02 1,26E+01 1,20E-01 0 4,09E+00 0 0
RWD kg 4,30E-02 1,76E-03 0,00E+00 0 5,57E-04 0 0
Indicator Unit B5 B6 B7 C1 C2 C3 C4 D
HWD kg 0 1,04E+01 0 1,86E-04 8,88E-03 5,01E-03 1,77E-01 9,87E-01
NHWD kg 0 4,80E+02 0 7,49E-03 8,38E+00 1,46E+00 6,89E+01 -2,21E+02
RWD kg 0 2,48E-01 0 4,39E-05 1,17E-03 5,79E-06 4,71E-05 -2,48E-02
HWD = Hazardous waste disposed; NHWD = Non-hazardous waste disposed; RWD = Radioactive waste disposed
"Reading example: 9,0 E-03 = 9,0*10-3 = 0,009"
*INA Indicator Not Assessed
End of life - Output flow
Indicator Unit A1-A3 A4 A5 B1 B2 B3 B4
CRU kg 0,00E+00 0,00E+00 0,00E+00 0 0,00E+00 0 0
MFR kg 5,95E+01 0,00E+00 6,13E-02 0 6,11E-05 0 0
MER kg 4,81E+00 0,00E+00 6,00E-06 0 1,16E+00 0 0
EEE MJ 3,66E+00 0,00E+00 9,22E-06 0 6,03E-01 0 0
EET MJ 5,54E+01 0,00E+00 1,39E-04 0 9,13E+00 0 0
Indicator Unit B5 B6 B7 C1 C2 C3 C4 D
CRU kg 0 0,00E+00 0 0,00E+00 0,00E+00 0,00E+00 0,00E+00 0,00E+00
MFR kg 0 0,00E+00 0 3,05E-03 0,00E+00 2,71E+02 1,89E-03 -9,08E-02
MER kg 0 0,00E+00 0 9,46E-06 0,00E+00 4,40E+00 2,68E-05 -1,20E-02
EEE MJ 0 0,00E+00 0 3,24E-05 0,00E+00 5,81E+00 9,34E-04 -2,93E-02
EET MJ 0 0,00E+00 0 4,91E-04 0,00E+00 8,79E+01 1,41E-02 -4,43E-01
CRU = Components for re-use; MFR = Materials for recycling; MER = Materials for energy recovery; EEE = Exported energy electrical; EET = Exported energy thermal
"Reading example: 9,0 E-03 = 9,0*10-3 = 0,009"
*INA Indicator Not Assessed
Biogenic Carbon Content
Indicator Unit At the factory gate
Biogenic carbon content in product kg C 0,00E+00
Biogenic carbon content in accompanying packaging kg C 0,00E+00
Note: 1 kg biogenic carbon is equivalent to 44/12 kg CO2
13 / 15
Additional requirements
Greenhouse gas emissions from the use of electricity in the manufacturing phase
National production mix from import, low voltage (production of transmission lines, in addition to direct emissions and losses in grid) of applied
electricity for the manufacturing process (A3).
Electricity mix Source Amount Unit
Electricity, Denmark (kWh) ecoinvent 3.6 338,20 g CO2-eq/kWh
Dangerous substances
The product contains no substances given by the REACH Candidate list.
Indoor environment
Additional Environmental Information
Additional environmental impact indicators required in NPCR Part A for construction products
Indicator Unit A1-A3 A4 A5 B1 B2 B3 B4
GWPIOBC kg CO2 -eq 2,52E+03 1,71E+01 9,51E-03 0 1,48E+01 0 0
Indicator Unit B5 B6 B7 C1 C2 C3 C4 D
GWPIOBC kg CO2 -eq 0 8,49E+03 0 4,60E-01 1,14E+01 2,37E+01 1,27E+00 -7,57E+02
GWP-IOBC: Global warming potential calculated according to the principle of instantaneous oxidation. In order to increase the transparency of biogenic carbon​
contribution to climate impact, the indicator GWP-IOBC is required as it declares climate impacts calculated according to the principle of instantaneous oxidation.​
GWP-IOBC is also referred to as GWP-GHG in context to Swedish public procurement legislation.
14 / 15
Bibliography
ISO 14025:2010 Environmental labels and declarations - Type III environmental declarations - Principles and procedures.
ISO 14044:2006 Environmental management - Life cycle assessment - Requirements and guidelines.
EN 15804:2012+A2:2019 Environmental product declaration - Core rules for the product category of construction products.
ISO 21930:2017 Sustainability in buildings and civil engineering works - Core rules for environmental product declarations of construction
products.
ecoinvent v3, Allocation, cut-off by classification, Swiss Centre of Life Cycle Inventories.
Iversen et al., (2021) eEPD v2021.09 Background information for EPD generator tool system verification, LCA.no Report number: 07.21
Graafland and Iversen (2022) EPD generator for NPCR 030 Ventilation components, Background information for EPD generator application and
LCA data, LCA.no report number: 12.22
NPCR Part A: Construction products and services. Ver. 2.0. April 2021, EPD-Norge.
NPCR 030 Part B for Ventilation components, Ver. 1.0, 18.05.2021, EPD Norway.
Program operator and publisher Phone: +47 977 22 020
The Norwegian EPD Foundation e-mail: post@epd-norge.no
Post Box 5250 Majorstuen, 0303 Oslo, Norway web: www.epd-norge.no
Owner of the declaration: Phone: +47 63 87 07 70
EXHAUSTO AS e-mail: lrr@exhausto.no
Hvamsvingen 4, 2013 Skjetten, Norway web: Exhausto.no
Author of the Life Cycle Assessment Phone: +47 916 50 916
LCA.no AS e-mail: post@lca.no
Dokka 6A, 1671 Kråkerøy, Norway web: www.lca.no
Developer of EPD generator Phone: +47 916 50 916
LCA.no AS e-mail: post@lca.no
Dokka 6A, 1671 Kråkerøy, Norway web: www.lca.no
ECO Platform web: www.eco-platform.org
ECO Portal web: ECO Portal
15 / 15
