Environmental product declaration
in accordance with ISO 14025 and EN 15804+A2
Vika Floor Screen without Lighting 427x1540x231
Owner of the declaration: Program operator:
Abstracta AB The Norwegian EPD Foundation
Product: Declaration number:
Vika Floor Screen without Lighting 427x1540x231
NEPD-6357-5615-EN
Declared unit:
1 pcs Registration number:
This declaration is based on Product Category Rules: NEPD-6357-5615-EN
CEN Standard EN 15804:2012+A2:2019 serves as core
Issue date: 04.04.2024
PCR
The Norwegian EPD Foundation
NPCR 026:2022 Part B for Furniture Valid to: 04.04.2029
EPD software:
LCAno EPD generator ID: 264583
1 / 12
General information
Product Owner of the declaration:
Vika Floor Screen without Lighting 427x1540x231 Abstracta AB
Contact person: Tim Wisme
Phone:
e-mail: tim.wisme@abstracta.se
Program operator: Manufacturer:
Post Box 5250 Majorstuen, 0303 Oslo, Norway Abstracta AB
The Norwegian EPD Foundation
Phone: +47 23 08 80 00
web: post@epd-norge.no
Declaration number: Place of production:
NEPD-6357-5615-EN Abstracta AB
Lammengatan 2
363 45 Lammhult, Sweden
This declaration is based on Product Category Rules: Management system:
CEN Standard EN 15804:2012+A2:2019 serves as core PCR ISO 9001, 14001 och 45001
NPCR 026:2022 Part B for Furniture
Statement of liability: Organisation no:
The owner of the declaration shall be liable for the underlying 556046-3852
information and evidence. EPD Norway shall not be liable with respect
to manufacturer information, life cycle assessment data and
evidences.​
Declared unit: Issue date:
1 pcs Vika Floor Screen without Lighting 427x1540x231 04.04.2024
Declared unit (cradle to gate) with option: Valid to:
A1-A3,A4,A5,B2,B3,B4,C1,C2,C3,C4,D 04.04.2029
Year of study:
2023
Functional unit: Comparability:
This EPD considers one pcs of Vika Floor Screen. The product is a EPD of construction products may not be comparable if they not
sound absorbing floor screen, with the possibility to add lighting. At comply with EN 15804 and seen in a building context.
the end of its life it can be dismantled and recycled or returned to
Abstracta for reuse or recycling.
General information on verification of EPD from EPD tools: Development and verification of EPD:
Independent verification of data, other environmental information The declaration is created using EPD tool lca.tools ver EPD2022.03,
and the declaration according to ISO 14025:2010, § 8.1.3 and § 8.1.4. developed by LCA.no. The EPD tool is integrated in the company's
Verification of each EPD is made according to EPD-Norway’s management system, and has been approved by EPD Norway.
guidelines for verification and approval requiring that tools are i)
integrated into the company's environmental management system, ii) Developer of EPD: Tim Wisme
the procedures for use of the EPD tool are approved by EPD-Norway,
Reviewer of company-specific input data and EPD: Erik Graesen
and iii) the process is reviewed annually by an independent third
party verifier. See Appendix G of EPD-Norway's General Programme
Instructions for further information on EPD tools
Verification of EPD tool: Approved:
Independent third party verification of the EPD tool, background data
and test-EPD in accordance with EPDNorway's procedures and
guidelines for verification and approval of EPD tools. Håkon Hauan, CEO EPD-Norge
Third party verifier:
Elisabet Amat, GREENIZE projects
(no signature required)
2 / 12
Product
Product description:
In collaboration with designer Khodi Feiz, Abstracta takes a new approach to acoustic lighting — one that aims to create a peaceful atmosphere.
The result is Vika, a sculptural floor screen that radiates atmospheric light while managing both low-frequency and high-frequency noise. “It’s
another way of thinking about sound and light,” says Feiz.
Vika can be used to divide a large space into smaller rooms, creating a better soundscape and a quieter atmosphere.
A clever thing about Vika is that both the floor screens and the ceiling luminaire are designed to be close to those in the room who are its sound
sources. This stops sound waves before they can bounce off the walls and ceiling.
For more information about the product, visit the product page https://abstracta.se/product/vika-acoustic-floor-screen-luminaire/
Product specification
Vika consists of a soft, sound-absorbing core, partly made of recycled PET bottles, and is covered with Texfel acoustic felt. Its base is made of black-
coated metal. Optionally available with lighting, however, these variants are not included in this EPD.
This EPD includes these variants:
Vika Floor Screen without Lighting 427x1540x231
Vika Floor Screen without Lighting 1180x1540x231
See the product sheet for more information: https://lammhults.sharepoint.com/:b:/s/abs-
webpage/ERhF4cCwy4lKgpee0cY6XWQBGsIaf9Klw5gZfSiSXZbmwA?e=pgtkjn
Recycled share in Recycled share in
Materials kg %
material (kg) material (%)
Adhesive 0,06 0,88 0,00 0,00
Filt 2,88 42,22 1,44 50,00
Metal - Aluminium 0,10 1,44 0,00 0,00
Metal - Stainless steel 0,06 0,82 0,01 21,83
Metal - Steel 2,69 39,51 0,00 0,00
Powder coating 0,02 0,28 0,00 0,00
Textile - Felt 1,01 14,74 0,90 90,00
Textile - Polyester (PE) 0,01 0,12 0,00 0,00
Total 6,82 2,36
Recycled share in Recycled share in
Packaging kg %
material (kg) material (%)
Recycled cardboard 1,93 100,00 1,93 100,00
Total incl. packaging 8,75 4,29
Technical data:
The dimensions of Vika Floor Screen without Lighting are 427x1540x231, but other sizes are also available. For more information on the technical
data of Vika Floor Screen, see the technical data sheet: https://lammhults.sharepoint.com/:b:/s/abs-
webpage/Ea58LrptusBBmk1FpWgvkqcBQAoU0JY7CBQN-eO3UoEJ3w?e=t5Qiz5.
Market:
The product is available worldwide. The distance to the market is based on shipping to Scandinavia or Western Europe.
Reference service life, product
At least 10 years, with a 5-year warranty and a 10-year spare part guarantee.
Reference service life, building
Assumed to be 60 years.
LCA: Calculation rules
Declared unit:
1 pcs Vika Floor Screen without Lighting 427x1540x231
Cut-off criteria:
All major raw materials and all the essential energy is included. The production processes for raw materials and energy flows with very small
amounts (less than 1%) are not included. These cut-off criteria do not apply for hazardous materials and substances.
Allocation:
3 / 12
The allocation is made in accordance with the provisions of EN 15804. Incoming energy and water and waste production in-house is allocated
equally among all products through mass allocation. Effects of primary production of recycled materials is allocated to the main product in which
the material was used. The recycling process and transportation of the material is allocated to this analysis.
Data quality:
Specific data for the product composition are provided by the manufacturer. They represent the production of the declared product and were
collected for EPD development in the year of study. Background data is based on registered EPDs according to EN 15804, Ostfold Research
databases, ecoinvent and other LCA databases. The data quality of the raw materials in A1 is presented in the table below.​
Materials Source Data quality Year
Adhesive ecoinvent 3.6 Database 2019
Filt S-P-04908 EPD 2020
Metal - Aluminium ecoinvent 3.6 database 2019
Metal - Stainless steel ecoinvent 3.6 Database 2019
Metal - Steel ecoinvent 3.6 Database 2019
Powder coating Ecoinvent 3.6 Database 2019
Recycled cardboard Modified ecoinvent 3.6 Database 2019
Textile - Felt S-P-11466 EPD 2023
Textile - Polyester (PE) ecoinvent 3.6 Database 2019
4 / 12
System boundaries (X=included, MND=module not declared, MNR=module not relevant)
Construction Beyond the system
Product stage Use stage End of life stage
installation stage boundaries
A1 A2 A3 A4 A5 B1 B2 B3 B4 B5 B6 B7 C1 C2 C3 C4 D
X X X X X MNR X X X MNR MNR MNR X X X X X
System boundary:
The EPD is a cradle-to-cradle analysis, A1-D, where some B-stages (use phase) that were assumed to be neglectable are not included.
The A1-A4 stages includes the extraction and production of raw materials, transportation to the production site, the production process itself, and
an estimated transport distance to the market. A5 includes the generated waste from the packaging of the product after assembly at the
customer.
The only B stage that is assumed to be relevant is B2. This stage includes assumptions on how the customer takes care of the product according to
Abstracta's care instructions.
The C- and D-stages includes the use of materials and energy for deconstruction, the transport to waste management, the waste processes,
disposal of materials that cannot be processed, and the potential of reuse, recovery, and recycling of the product.
Additional technical information:
To preserve the fabric colour and the appearance of the fabric, Vika should be vacuumed regularly with a soft nozzle.
Polyester Stain Removal: Use uncoloured paper towel or cloth to soak up as much as possible of the stain. Dried stains should be vacuumed.
Moisten the stain lightly with a clean white cotton cloth, lukewarm water and possibly a small amount of pH-neutral detergent. Press a dry cloth
or uncoloured paper towel against the fabric so that moisture and dirt are absorbed. Repeat moistening and soaking until the stain is gone. Use
clean water without detergent at the last moistening. Finish with soaking.
Abstracta offers a reuse service for our clients. This involves us collecting worn-out products to facilitate reuse, renovation, or recycling. In order to
make circularity easier, most of our products feature replaceable parts, simplifying repair. We do this in the hope that we can help contribute in the
transition to a more sustainable future. Read more about the service here: https://abstracta.se/story/abstracta-is-introducing-a-new-recycling-
service-for-used-products-abstracta/ or contact our Sales Support for more information. Otherwise, try to ensure that the product can be reused
when possible, or else, dismantle it so that as much of the materials can be recycled as possible.
waR slairetam tropsnarT gnirutcafunaM tropsnarT ylbmessA e​sU ecnanetniaM riapeR tnemecalpeR tnemhsibrufeR lanoitarepO ygrene esu lanoitarepO esu retaw -eD noitcurtsnoc noitilomed tropsnarT etsaW gnissecorp lasopsiD -yrevoceR-esueR laitnetop-gnilcyceR
5 / 12
LCA: Scenarios and additional technical information
The following information describe the scenarios in the different modules of the EPD.
Some assumptions have been made regarding the products lifetime after leaving the factory gates. The product is assumed to be transported to a
customer in Scandinavia, Germany, the UK, or France (88% of sales in 2023). An average distance to the customer has been calculated through
this data. In the A5 phase, the packaging of the product becomes waste, and the impacts are added automatically according to assumptions made
in the EPD tool on waste handling on-site. In the use stage, the assumption is that the customer takes care of the product by vacuuming it for 1
minute/m2 of the product, with a 600 W vacuum, on a yearly basis. For the end-of-life stage of the product, it has been assumed that there is a
50 km distance from the customer to a waste terminal. The rest of the values are automatically filled in by the tool. For the D-stage, automatic
values are filled in, according to generic data.
Capacity utilisation Value
Transport from production place to user (A4) Distance (km) Fuel/Energy Consumption Unit
(incl. return) % (Liter/tonne)
Ship, Ferry, Sea (km) 50,0 % 8 0,034 l/tkm 0,27
Truck, 16-32 tonnes, EURO 6 (km) 36,7 % 502 0,043 l/tkm 21,58
Assembly (A5) Unit Value
Waste, packaging, cardboard, 100 % recycled, to
kg 1,93
average treatment (kg)
Maintenance (B2) Unit Value
Electricity, Nordic (kWh) kWh/DU 0,20
Capacity utilisation Value
Transport to waste processing (C2) Distance (km) Fuel/Energy Consumption Unit
(incl. return) % (Liter/tonne)
Truck, 16-32 tonnes, EURO 6 (km) 36,7 % 50 0,043 l/tkm 2,15
Waste processing (C3) Unit Value
Waste treatment per kg Hazardous waste,
kg 0,06
incineration (kg)
Waste treatment per kg Non-hazardous waste,
kg 0,02
incineration with fly ash extraction - C3 (kg)
Waste treatment per kg Polyethylene
terephthalate, PET, incineration with fly ash kg 2,88
extraction - C3 (kg)
Waste treatment per kg Scrap aluminium,
kg 0,10
incineration with fly ash extraction (kg)
Waste treatment per kg Scrap steel, incineration
kg 2,75
with fly ash extraction (kg)
Waste treatment per kg Textile, incineration with
kg 1,01
fly ash extraction (kg)
Waste, materials to recycling (kg) kg 0,94
Disposal (C4) Unit Value
Landfilling of ashes and residues from
kg 0,09
incineration of Scrap aluminium (kg)
Landfilling of ashes and residues from
kg 1,82
incineration of Scrap steel (kg)
Landfilling of ashes from incineration of
kg 0,01
Hazardous waste, from incineration (kg)
Landfilling of ashes from incineration of Non-
hazardous waste, process per kg ashes and kg 0,00
residues - C4 (kg)
Landfilling of ashes from incineration of
Polyethylene terephthalate, PET, process per kg kg 0,06
ashes and residues - C4 (kg)
Landfilling of ashes from incineration of Textile,
kg 0,05
soiled, process per kg ashes and residues (kg)
Benefits and loads beyond the system
Unit Value
boundaries (D)
Substitution of electricity, in Norway (MJ) MJ 3,95
Substitution of primary aluminium with net scrap
kg 0,01
(kg)
Substitution of primary steel with net scrap (kg) kg 0,93
Substitution of thermal energy, district heating, in
MJ 59,82
Norway (MJ)
6 / 12
LCA: Results
The LCA results are presented below for the declared unit defined on page 2 of the EPD document.
Environmental impact
Indicator Unit A1-A3 A4 A5 B2 B3
GWP-total kg CO2 -eq 2,12E+01 7,26E-01 3,31E+00 2,91E-02 0
GWP-fossil kg CO2 -eq 2,36E+01 7,25E-01 3,13E-02 2,72E-02 0
GWP-biogenic kg CO2 -eq -2,46E+00 2,99E-04 3,28E+00 4,96E-04 0
GWP-luluc kg CO2 -eq 5,35E-02 2,60E-04 1,03E-05 1,49E-03 0
ODP kg CFC11 -eq 1,51E-05 1,64E-07 6,60E-09 2,94E-09 0
AP mol H+ -eq 1,17E-01 2,31E-03 1,48E-04 1,25E-04 0
EP-FreshWater kg P -eq 2,53E-03 5,76E-06 2,57E-07 1,80E-06 0
EP-Marine kg N -eq 2,61E-02 4,71E-04 4,89E-05 1,98E-05 0
EP-Terrestial mol N -eq 2,65E-01 5,26E-03 5,30E-04 2,66E-04 0
POCP kg NMVOC -eq 1,02E-01 1,93E-03 1,52E-04 6,22E-05 0
ADP-minerals&metals1 kg Sb-eq 3,66E-04 1,99E-05 7,61E-07 4,22E-07 0
ADP-fossil1 MJ 3,49E+02 1,09E+01 4,37E-01 7,34E-01 0
WDP1 m3 1,75E+03 1,05E+01 5,54E-01 5,67E+01 0
Indicator Unit B4 C1 C2 C3 C4 D
GWP-total kg CO2 -eq 0 0 7,15E-02 7,62E+00 2,91E-02 -1,47E+00
GWP-fossil kg CO2 -eq 0 0 7,15E-02 6,14E+00 2,91E-02 -1,46E+00
GWP-biogenic kg CO2 -eq 0 0 2,96E-05 1,48E+00 2,56E-05 -1,70E-03
GWP-luluc kg CO2 -eq 0 0 2,54E-05 4,85E-05 7,35E-06 -1,41E-02
ODP kg CFC11 -eq 0 0 1,62E-08 2,40E-08 7,15E-09 -2,53E-02
AP mol H+ -eq 0 0 2,05E-04 1,59E-03 1,71E-04 -8,55E-03
EP-FreshWater kg P -eq 0 0 5,71E-07 4,46E-06 2,98E-07 -9,72E-05
EP-Marine kg N -eq 0 0 4,06E-05 7,52E-04 5,95E-05 -2,06E-03
EP-Terrestial mol N -eq 0 0 4,55E-04 7,67E-03 6,61E-04 -2,17E-02
POCP kg NMVOC -eq 0 0 1,74E-04 1,89E-03 1,89E-04 -8,19E-03
ADP-minerals&metals1 kg Sb-eq 0 0 1,97E-06 8,69E-07 3,93E-07 -2,09E-05
ADP-fossil1 MJ 0 0 1,08E+00 1,37E+00 5,37E-01 -1,47E+01
WDP1 m3 0 0 1,05E+00 2,91E+00 1,82E+00 -6,05E+01
GWP-total = Global Warming Potential total; GWP-fossil = Global Warming Potential fossil fuels; GWP-biogenic = Global Warming Potential biogenic; GWP-luluc =
Global Warming Potential land use and land use change; ODP = Depletion potential of the stratospheric ozone layer; AP = Acidification potential, Accumulated
Exceedance; EP-freshwater = Eutrophication potential, fraction of nutrients reaching freshwater end compartment: EP-marine = Eutrophication potential, fraction of
nutrients reaching marine end compartment; EP-terrestrial = Eutrophication potential, Accumulated Exceedance; POCP = Formation potential of tropospheric ozone;
ADP-minerals&metals = Abiotic depletion potential for non-fossil resources; ADP-fossil = Abiotic depletion for fossil resources potential; WDP = Water (user)
deprivation potential, deprivation-weighted water consumption
"Reading example: 9,0 E-03 = 9,0*10-3 = 0,009"
*INA Indicator Not Assessed
1. The results of this environmental impact indicator shall be used with care as the uncertainties on these results are high or as there is limited experienced with the
indicator
Remarks to environmental impacts
7 / 12
Additional environmental impact indicators
Indicator Unit A1-A3 A4 A5 B2 B3
PM Disease incidence 1,57E-06 4,41E-08 2,18E-09 6,64E-10 0
IRP2 kgBq U235 -eq 1,60E+00 4,78E-02 1,87E-03 1,67E-02 0
ETP-fw1 CTUe 1,22E+03 8,10E+00 5,83E-01 9,19E-01 0
HTP-c1 CTUh 8,52E-08 0,00E+00 1,70E-11 2,10E-11 0
HTP-nc1 CTUh 5,76E-07 8,85E-09 7,32E-10 5,64E-10 0
SQP1 dimensionless 1,34E+02 7,60E+00 2,93E-01 5,53E-01 0
Indicator Unit B4 C1 C2 C3 C4 D
PM Disease incidence 0 0 4,38E-09 1,56E-08 2,95E-09 -2,64E-07
IRP2 kgBq U235 -eq 0 0 4,72E-03 4,03E-03 2,21E-03 -3,30E-02
ETP-fw1 CTUe 0 0 8,01E-01 5,67E+00 4,02E-01 -8,53E+01
HTP-c1 CTUh 0 0 0,00E+00 4,63E-10 1,60E-11 -5,64E-09
HTP-nc1 CTUh 0 0 8,75E-10 1,21E-08 4,92E-10 7,83E-08
SQP1 dimensionless 0 0 7,56E-01 3,33E-01 1,20E+00 -3,38E+01
PM = Particulate Matter emissions; IRP = Ionizing radiation – human health; ETP-fw = Eco toxicity – freshwater; HTP-c = Human toxicity – cancer effects; HTP-nc =
Human toxicity – non cancer effects; SQP = Soil Quality (dimensionless)
"Reading example: 9,0 E-03 = 9,0*10-3 = 0,009"
*INA Indicator Not Assessed
1. The results of this environmental impact indicator shall be used with care as the uncertainties on these results are high or as there is limited experienced with the
indicator
2. This impact category deals mainly with the eventual impact of low dose ionizing radiation on human health of the nuclear fuel cycle. It does not consider effects due
to possible nuclear accidents, occupational exposure nor due to radioactive waste disposal in underground facilities. Potential ionizing radiation from the soil, from
radon and from some construction materials is also not measured by this indicator.
8 / 12
Resource use
Indicator Unit A1-A3 A4 A5 B2 B3
PERE MJ 6,68E+01 1,56E-01 7,20E-03 7,22E-01 0
PERM MJ 1,88E+01 0,00E+00 -1,13E+01 0,00E+00 0
PERT MJ 8,56E+01 1,56E-01 -1,13E+01 7,22E-01 0
PENRE MJ 2,95E+02 1,09E+01 4,37E-01 7,45E-01 0
PENRM MJ 6,04E+01 0,00E+00 0,00E+00 0,00E+00 0
PENRT MJ 3,56E+02 1,09E+01 4,37E-01 7,45E-01 0
SM kg 4,29E+00 0,00E+00 0,00E+00 0,00E+00 0
RSF MJ 1,46E-01 5,57E-03 2,39E-04 7,29E-03 0
NRSF MJ 8,26E-02 1,99E-02 9,84E-04 0,00E+00 0
FW m3 1,99E-01 1,16E-03 2,06E-04 3,28E-03 0
Indicator Unit B4 C1 C2 C3 C4 D
PERE MJ 0 0 1,55E-02 1,26E-01 1,34E-02 -3,17E+01
PERM MJ 0 0 0,00E+00 0,00E+00 0,00E+00 0,00E+00
PERT MJ 0 0 1,55E-02 1,26E-01 1,34E-02 -3,17E+01
PENRE MJ 0 0 1,08E+00 1,39E+00 5,37E-01 -1,47E+01
PENRM MJ 0 0 0,00E+00 -6,04E+01 0,00E+00 0,00E+00
PENRT MJ 0 0 1,08E+00 -5,90E+01 5,37E-01 -1,47E+01
SM kg 0 0 0,00E+00 0,00E+00 0,00E+00 0,00E+00
RSF MJ 0 0 5,53E-04 2,83E-03 3,28E-04 3,14E-02
NRSF MJ 0 0 1,98E-03 0,00E+00 2,16E-02 -7,41E-01
FW m3 0 0 1,16E-04 1,99E-03 5,05E-04 -4,13E-02
PERE = Use of renewable primary energy excluding renewable primary energy resources used as raw materials; PERM = Use of renewable primary energy resources used
as raw materials; PERT = Total use of renewable primary energy resources; PENRE = Use of non renewable primary energy excluding non-renewable primary energy
resources used as raw materials; PENRM = Use of non renewable primary energy resources used as raw materials; PENRT = Total use of non renewable primary energy
resources; SM = Use of secondary materials; RSF = Use of renewable secondary fuels; NRSF = Use of non-renewable secondary fuels; FW = Net use of fresh water
"Reading example: 9,0 E-03 = 9,0*10-3 = 0,009"
*INA Indicator Not Assessed
9 / 12
End of life - Waste
Indicator Unit A1-A3 A4 A5 B2 B3
HWD kg 1,87E-01 5,63E-04 0,00E+00 6,88E-05 0
NHWD kg 5,91E+00 5,28E-01 1,93E+00 4,56E-03 0
RWD kg 7,49E-04 7,46E-05 0,00E+00 7,69E-06 0
Indicator Unit B4 C1 C2 C3 C4 D
HWD kg 0 0 5,57E-05 0,00E+00 1,95E+00 -5,17E-03
NHWD kg 0 0 5,26E-02 7,90E-02 5,34E-02 -5,61E-01
RWD kg 0 0 7,36E-06 0,00E+00 3,16E-06 -2,78E-05
HWD = Hazardous waste disposed; NHWD = Non-hazardous waste disposed; RWD = Radioactive waste disposed
"Reading example: 9,0 E-03 = 9,0*10-3 = 0,009"
*INA Indicator Not Assessed
End of life - Output flow
Indicator Unit A1-A3 A4 A5 B2 B3
CRU kg 0,00E+00 0,00E+00 0,00E+00 0,00E+00 0
MFR kg 6,63E-02 0,00E+00 1,80E+00 0,00E+00 0
MER kg 2,11E-01 0,00E+00 2,63E-06 0,00E+00 0
EEE MJ 1,30E-01 0,00E+00 1,11E-01 0,00E+00 0
EET MJ 1,96E+00 0,00E+00 1,67E+00 0,00E+00 0
Indicator Unit B4 C1 C2 C3 C4 D
CRU kg 0 0 0,00E+00 0,00E+00 0,00E+00 0,00E+00
MFR kg 0 0 0,00E+00 9,43E-01 0,00E+00 0,00E+00
MER kg 0 0 0,00E+00 6,82E+00 0,00E+00 0,00E+00
EEE MJ 0 0 0,00E+00 3,81E+00 0,00E+00 0,00E+00
EET MJ 0 0 0,00E+00 5,76E+01 0,00E+00 0,00E+00
CRU = Components for re-use; MFR = Materials for recycling; MER = Materials for energy recovery; EEE = Exported energy electrical; EET = Exported energy thermal
"Reading example: 9,0 E-03 = 9,0*10-3 = 0,009"
*INA Indicator Not Assessed
Biogenic Carbon Content
Indicator Unit At the factory gate
Biogenic carbon content in product kg C 0,00E+00
Biogenic carbon content in accompanying packaging kg C 1,07E+00
Note: 1 kg biogenic carbon is equivalent to 44/12 kg CO2
10 / 12
Additional requirements
Greenhouse gas emissions from the use of electricity in the manufacturing phase
National production mix from import, low voltage (production of transmission lines, in addition to direct emissions and losses in grid) of applied
electricity for the manufacturing process (A3).
Electricity mix Data source Amount Unit
Electricity, Sweden (kWh) ecoinvent 3.6 54,94 g CO2-eq/kWh
Dangerous substances
The product contains no substances given by the REACH Candidate list.
Indoor environment
A test for the indoor emissions is available here: https://lammhults.sharepoint.com/:b:/s/abs-
webpage/Ec_jJut4HDlOn05QeqhowbwByeAsjf1W6xP55qQZJ1uqAg?e=83tDuL
Additional Environmental Information
Key Environmental Indicators
Key environmental indicators Unit A1-A3 A4 A1-C4 A1-D
GWPtotal kg CO2 -eq 21,22 0,73 33,01 31,53
Total energy consumption MJ 362,53 11,13 378,76 331,59
Amount of recycled materials % 42,96
Additional environmental impact indicators required in NPCR Part A for construction products
Indicator Unit A1-A3 A4 A5 B2 B3
GWPIOBC kg CO2 -eq 2,41E+01 7,26E-01 3,13E-02 3,95E-02 0
Indicator Unit B4 C1 C2 C3 C4 D
GWPIOBC kg CO2 -eq 0 0 7,15E-02 7,77E+00 3,23E-02 -1,97E+00
GWP-IOBC: Global warming potential calculated according to the principle of instantaneous oxidation. In order to increase the transparency of biogenic carbon
contribution to climate impact, the indicator GWP-IOBC is required as it declares climate impacts calculated according to the principle of instantaneous oxidation.
GWP-IOBC is also referred to as GWP-GHG in context to Swedish public procurement legislation.
Variants and Options
Key environmental indicators (A1-A3) for variants of this EPD
Variants Weight (kg) GWPtotal (kg CO2 -eq) Total energy consumption (MJ) Amount of recycled materials (%)
Vika Floor Screen without Lighting 1180x1540x231 26,60 64,81 1109,60 49,04
11 / 12
Bibliography
ISO 14025:2010 Environmental labels and declarations - Type III environmental declarations - Principles and procedures.
ISO 14044:2006 Environmental management - Life cycle assessment - Requirements and guidelines.
EN 15804:2012+A2:2019 Environmental product declaration - Core rules for the product category of construction products.
ISO 21930:2017 Sustainability in buildings and civil engineering works - Core rules for environmental product declarations of construction
products.
ecoinvent v3, Allocation, cut-off by classification, Swiss Centre of Life Cycle Inventories.
Iversen et al., (2021) eEPD v2021.09 Background information for EPD generator tool system verification, LCA.no Report number: 07.21
Ruud et al., (2023) EPD generator for NPCR026 Part B for Furniture - Background information for EPD generator application and LCA data,
LCA.no report number 01.23
NPCR Part A: Construction products and services. Ver. 2.0. March 2021, EPD-Norge.
NPCR 026 Part B for Furniture. Ver. 2.0 March 2022, EPD-Norge.
Program operator and publisher Phone: +47 23 08 80 00
The Norwegian EPD Foundation e-mail: post@epd-norge.no
Post Box 5250 Majorstuen, 0303 Oslo, Norway web: www.epd-norge.no
Owner of the declaration: Phone:
Abstracta AB e-mail: tim.wisme@abstracta.se
Lammengatan 2, 363 45 Lammhult web: www.abstracta.se
Author of the Life Cycle Assessment Phone: +47 916 50 916
LCA.no AS e-mail: post@lca.no
Dokka 6B, 1671 web: www.lca.no
Developer of EPD generator Phone: +47 916 50 916
LCA.no AS e-mail: post@lca.no
Dokka 6B,1671 Kråkerøy web: www.lca.no
ECO Platform web: www.eco-platform.org
ECO Portal web: ECO Portal
12 / 12
