ENVIRONMENTAL PRODUCT DECLARATION
as per ISO 14025 and EN 15804+A2
Owner of the Declaration IGI - The Global Wallcoverings Association
Publisher Institut Bauen und Umwelt e.V. (IBU)
Programme holder Institut Bauen und Umwelt e.V. (IBU)
Declaration number EPD-IGI-20230437-IBG1-EN
Issue date 18.01.2024
Valid to 17.01.2029
Vinyl wallcoverings on cellulose fibre base
IGI - The Global Wallcoverings Association
www.ibu-epd.com | https://epd-online.com
1. General Information
IGI - The Global Wallcoverings Association Vinyl wallcoverings on cellulose fibre base
Programme holder Owner of the declaration
IBU – Institut Bauen und Umwelt e.V. IGI - The Global Wallcoverings Association
Hegelplatz 1 Chaussée de Louvain 426
10117 Berlin 1380 LASNE
Germany Belgium
Declaration number Declared product / declared unit
EPD-IGI-20230437-IBG1-EN The declared unit is 1m² (square meter) decorative vinyl wallcovering on
cellulose fibre base including packaging.
This declaration is based on the product category rules: Scope:
Wall coverings, 01.08.2021 This EPD focusses on the production, transport and disposal of a weighted
(PCR checked and approved by the SVR) average of 1m² vinyl wallcoverings on cellulose fibre base of participating
members of the IGI - The Global Wallcoverings Association.
12 out of 71 IGI-members are involved in this EPD: A.S. Création Tapeten
Issue date AG (DE), Anstey Wallpaper Co. Ltd (GB), BN International (NL), Erismann
& Cie. GmbH (DE), Graham & Brown Ltd (GB), Grandeco NV (BE), JV
18.01.2024
S.p.A. (IT), Marburger Tapetenfabrik J.B. Schaefer GmbH & Co. KG (DE),
Muraspec Decorative Solutions Ltd (GB), Rasch GmbH & Co. KG (DE),
UGÉPA SA (FR), Zambaiti Parati S.p.A. (IT).
Valid to
The technical properties are displayed in chapter 2.3.
17.01.2029 The owner of the declaration shall be liable for the underlying information
and evidence; the IBU shall not be liable with respect to manufacturer
information, life cycle assessment data and evidences.
The EPD was created according to the specifications of EN 15804+A2. In
the following, the standard will be simplified as EN 15804.
Verification
The standard EN 15804 serves as the core PCR
Independent verification of the declaration and data according to ISO
14025:2011
Dipl.-Ing. Hans Peters internally X externally
(Chairman of Institut Bauen und Umwelt e.V.)
Florian Pronold Prof. Dr. Birgit Grahl,
(Managing Director Institut Bauen und Umwelt e.V.) (Independent verifier)
1 Environmental Product Declaration - IGI - The Global Wallcoverings Association - Vinyl wallcoverings on cellulose fibre base
2. Product
2.1 Product description/Product definition or:
Vinyl wallcoverings on cellulose fibre base according to EN
15102 involve plasticized PVC (vinyl) and a cellulose fibre 1b
base. When the wallcovering is to be changed it can be Performance Category I, II, III, IV, V or VI as described in Table
delaminated from the wall. EN 235 defines delamination as 1 of F 793-0-06 should be declared.
peelable.
For the placing on the market of the product in the European 2.4 Delivery status
Union/European Free Trade Association (EU/EFTA) (with the The products declared are provided within the following
exception of Switzerland) Regulation (EU) No. 305/2011 (CPR) dimensions:
applies. The product needs a Declaration of Performance
taking into consideration EN 15102 and CE-marking. For the
application and use the respective national provisions apply.
For the placing on the market in Great Britain the product
needs a Declaration of Performance taking into consideration
BS EN 15102 and UK Conformity Assessed (UKCA) marking.
This table contains the range of all wallcoverings examined. For
more precise information please contact the specific
For placing on the market in Northern Ireland the product needs
manufacturer.
a Declaration of Performance taking into consideration (BS) EN
15102 and CE or CE and UK Northern Ireland (UKNI) marking. 2.5 Base materials/Ancillary materials
The weighted average of the primary product components is
For the placing on the market in the USA the product should shown in the following table, in percentage:
conform to ASTM F 1141 – 93 Standard Specification for
Name Value Unit
Wallcovering and ASTM F 793 – 06 Standard Classification of
Carrier material (Paper) 33 %
Wall Covering by Use Characteristics.
Packaging 11 %
2.2 Application
PVC plastisol 31 %
Wallcoverings are used for the decorative wall design of interior
Additives 22 %
spaces in private or commercial use.
Ink & Pigment 4 %
2.3 Technical Data Sum 100 %
Constructional data
Pallets were considered as part of the packaging.
In accordance with EN 233, the following technical (structural)
data can be declared on delivery: This product contains substances listed in the candidate list
Name Value Unit (date: 06.12.2023) exceeding 0.1 percentage by mass: yes,
Measures by categories EN 233 category 1 - 3 - C14-C17 chlorinated paraffin (containing < 1 % C10-13)
Straightness and parallelism in mm. equal or less than (chlorination: 40 - 63 %) CAS no.: 85535-85-9.
according to EN 12956 1 - This product contains other CMR substances in categories 1A
or 1B that are not on the candidate list, exceeding 0.1
spongeable to
Washability according to EN 12956 - percentage by mass: no.
extra-scrubbable
Biocide products were added to this construction product or it
Colour fastness to light according to
3 - 6 - has been treated with biocide products (this then concerns a
EN ISO 105-B02
treated product as defined by the (EU) Ordinance on Biocide
Migration of heavy metals and certain Products No. 528/2012): no.
fulfills the norm -
other elements to EN 12149 Ancillary materials of the phthalate chemical group, specifically
Vinyl chloride monomer (VCM) Diisononyl phthalate (DINP) and Dioctyl Terephthalate (DOTP),
content max. < 0,2 mg/m² according to fulfills the norm - remain on the product and serve the function of softeners.
EN 12149 Plasticizers can also be found in the products, in the plastisol
Emissions of formaldehyde max. used for vinyl finishing.
fulfills the norm -
< 120 mg/kg according to EN 12149 This EPD is a weighted average of a Manufacturer Group
regarding several producers and product references. Therefore,
In case of multiple answers, values need to be examined
it cannot be ruled out that individual wallcoverings may contain
depending on the manufacturer.
small amounts (>0.1% of product weight) of substances that
For USA manufactured products should be in accordance with
are included in the Substance of Very High Concern SVHC
ASTM F 793-0-06 Table 1 Classification Criteria.
candidate list, the CMR substances in categories 1A or 1B list
or ancillary materials and additives serving the function of fire
Depending on whether products are intended for the European,
retardants, softeners or biocides.
UK or US market, the following performance data must be
This can be attributed, for example, to the contents of used
declared.
waste paper. Further information can be obtained from the
respective manufacturer.
1a: Product
according to the CPR, based on (BS) EN 15102: 2.6 Manufacture
The manufacturing process can be described with the help of
Performance data of the product in accordance with the the following graphic:
Declaration of Performance with respect to its Essential
Characteristics according to EN 15102.
2 Environmental Product Declaration - IGI - The Global Wallcoverings Association - Vinyl wallcoverings on cellulose fibre base
Given the wallcovering is professionally installed, the reference
service life is 10 years according to the German Sustainable
Building Assessment System (BNB).
Description of the influences on the ageing of the product when
applied in accordance with the rules of technology.
2.13 Extraordinary effects
Fire
The reaction to fire performance according to EN 13501 is
shown in the following table:*
Name Value
Building material class B-D
Burning droplets s1-s3
Smoke gas development d0-d2
The order of manufacture may change and can slightly deviate *This table contains the range of all wallcoverings examined.
for different producers. For more precise information please contact the specific
manufacturer.
2.7 Environment and health during manufacturing For USA information on fire performance according to ASTM E
Compliance with statutory health and safety for personnel is 84 Test method for Surface Burning Characteristics of Building
ensured. Further, the energy and environmental management Materials.
is certified for some members according to ISO 14001 and ISO
50001.
For greater detail please contact the specific manufacturer. Water
The product is not water resistant. There is no risk of a
2.8 Product processing/Installation
hazardous environmental impact in the event of water flooding.
Depending on the manufacturers suggestion, the adhesive is
applied to the back of the wallcovering or the substrate using a Mechanical destruction
wallpaper brush or short-napped roller. The wallcovering is There is no risk of a hazardous environmental impact following
pressed against the wall and is cut along the top and bottom unforeseen mechanical destruction.
edges to fit the wall.
2.14 Re-use phase
2.9 Packaging
The product is not re-usable.
Product is wrapped in shrink-wrap clear film, packed in
corrugated cardboard boxes and palletised. 2.15 Disposal
Wallcoverings are subject to the waste code 170904 (mixed
2.10 Condition of use
construction and demolition waste other than those mentioned
There are no special features to be noted within the limits of in 170901, 170902 and 170903) in accordance with the
normal and customary usage. European Waste Catalogue (EWC).
Wallcoverings can therefore be disposed of as normal
2.11 Environment and health during use
household waste, that is in the dustbin or in additional refuse
No environmental problems can be expected when the product
sacks. Used wallcoverings should not be placed in the waste
is handled and used
paper bank. Most household waste is incinerated or landfilled
properly.
depending on regional legal regulations in the EU or in the US.
2.12 Reference service life
2.16 Further information
For further information please visit www.igiwallcoverings.org.
3. LCA: Calculation rules
3.1 Declared Unit 3.2 System boundary
The declared unit is 1 m² of wallcovering including packaging. Type of the EPD: cradle to gate - with option. The EPD is
The model is based on a weighted average of the produced considered a declaration of an average product as calculated
square meters of each participating manufacturer. from the output of several manufacturers (2b).
Declared unit
Modules A1-3, A4 and A5
Name Value Unit
The product stage begins with the consideration of the
Declared unit 1 m2 production of the necessary raw materials and energies
Grammage 0.251 kg/m2 including all corresponding upstream processes as well as
transport.
Conversion factor to 1 kg 3.982 -
Furthermore, the entire production phase was investigated,
Layer thickness 0.001 m
including the treatment of production waste until reaching the
Density 2511 kg/m3 end-of-waste status (EoW). In addition, distribution transport
The production processes and location may vary between and installation in the building were taken into account.
individual companies. The weighted average represents the
most likely scenario by production volumes and the selected Modules C1-4
datasets correspond to all regarded regions. The modules include the environmental impacts of the removal
and waste treatment until reaching the end-of-waste status
3 Environmental Product Declaration - IGI - The Global Wallcoverings Association - Vinyl wallcoverings on cellulose fibre base
(EoW) including the associated transport at the end of the environmental data, the collection of LCA-relevant data within
product life cycle. the supply chain as well as through the measurement of
relevant energy supply data. The collected data was checked
Module D for plausibility and consistency. A good representation is to be
Calculation of potential benefits through the generated energy assumed. The data were collected in 2022 and refer to the
(electric & thermic) by the incineration processes in the life calendar year 2021.
cycle stages in A5 C3 and C4. The burdens resulting from the
waste-to-energy plants are assigned in module C3 or C4 in 3.7 Period under review
case of landfill gas combustion. The LCA data were collected for the calendar year 2021.
3.3 Estimates and assumptions 3.8 Geographic Representativeness
Most solvents were modelled as a generic mix of solvents. Land or region, in which the declared product system is
manufactured, used or handled at the end of the product´s
3.4 Cut-off criteria lifespan: Global
No materials were cut-off from the study. No energy
consumption was neglected.
3.9 Allocation
3.5 Background data Potential benefits resulting from the thermal utilization of the
For modelling the lifecycle, the LCA for Experts Software packaging waste (module A5) as well as from the thermal
System and Database for Life Cycle Engineering (GaBi) utilization or landfilling of the wallcoverings at the end of life
Service pack 2023.1 was used. All background data records (modules C3 and C4) are allocated to module D.
relevant for production and disposal were almost exclusively
3.10 Comparability
taken from various GaBi supplementary databases or rarely
also from ecoinvent (v.3.6). The data records included in the Basically, a comparison or an evaluation of EPD data is only
databases are documented online. possible if all the data sets to be compared were created
according to EN 15804 and the building context, respectively
3.6 Data quality the product-specific characteristics of performance, are taken
Data collection for the investigated products was carried out on into account. The used background database is GaBi service
the basis of evaluations of the internal production and package 1 of 2023.
4. LCA: Scenarios and additional technical information
Name Value Unit
Characteristic product properties of biogenic carbon
Gross density of products transported - kg/m3
The biogenic carbon content quantifies the amount of biogenic
carbon in a construction product leaving the factory gate, and it Truck transport 27 t payload
is separately declared for the product and for any Transport distance 456 km
accompanying packaging. 1 kg of biogenic Carbon is Train transport 726 t payload
equivalent to 44/12 kg of CO .
2 Transport distance 16 km
Information on describing the biogenic Carbon Content at Ship transport 27500 dwt payload
factory gate Transport distance 156 km
Name ValueUnit Cargo plane transport 65 t payload
kg Transport distance 15 km
Biogenic carbon content in product 0.028
C Capacity utilisation (including empty runs) 80 - 90 %
Biogenic carbon content in accompanying kg
0.007 Because many different countries are involved, there were
packaging C
always global data sets used to model the transport distances.
Note: 1 kg of biogenic carbon is equivalent to 44/12 kg of CO .
2
Installation into the building (A5)
The treatment of packaging as waste was modeled in Module
The treatment of packaging as waste was modelled in Module
A5 as a weighted average. The following table depicts the
A5 as a weighted average.
packaging materials treated in A5 with more than 1 gram of
participation in the weighted average.
Modules B1-B7 are deemed not relevant since the product
Modules B1-B7 are deemed not relevant since the product
needs no maintenance or operational energy or water use and
needs no maintenance or operational energy or water use and
are therefore, not declared.
are, therefore, not declared.
Transport to the building site (A4) Name Value Unit
Cardboard 0.019 kg
Pallet 0.005 kg
Polyethylene 0.003 kg
Paper 0.001 kg
Reference service life
Name Value Unit
Reference service life 10 a
End of life (C1-C4)
4 Environmental Product Declaration - IGI - The Global Wallcoverings Association - Vinyl wallcoverings on cellulose fibre base
Name Value Unit Reuse, recovery and/or recycling potentials (D), relevant
scenario information
Incineration 100 %
In module D the potential benefits of the thermal combustion of
For the calculation of this LCA landfilling is chosen for the US the wallcoverings (C3) and their packaging (A5) are displayed.
and incineration for the EU. Different disposal routes are From the total paper used as backing, 25.2% of recycled paper
available but not taken into account for this industry average in the average product does not receive benefits, as it is a
LCA. secondary material coming burden-free to the system.
5 Environmental Product Declaration - IGI - The Global Wallcoverings Association - Vinyl wallcoverings on cellulose fibre base
5. LCA: Results
In this section, the LCA results for 1 m² wallcoverings are presented. It should be borne in mind that the LCA results only indicate
possible effects.
Indicators used for evaluation:
The EN 15804+A2 LCIA methodology with the characterization factors infrom EU-JRC were used to evaluate the possible
environmental effects of the wallcoverings. The characterization factors are available at the following internet link:
http://eplca.jrc.ec.europa.eu/LCDN/developerEF.xhtml.
DESCRIPTION OF THE SYSTEM BOUNDARY (X = INCLUDED IN LCA; MND = MODULE OR INDICATOR NOT DECLARED; MNR
= MODULE NOT RELEVANT)
Benefits and
Construction loads beyond
Product stage Use stage End of life stage
process stage the system
boundaries
la ire ta m w a Ry lp p u s tro p s n a rT g n iru tc a fu n a M e h t m o rf tro p s n a rTe tis e h t o t e ta g y lb m e s s A e s U e c n a n e tn ia M ria p e R tn e m e c a lp e R tn e m h s ib ru fe R y g re n e la n o ita re p Oe s u re ta w la n o ita re p Oe s u n o itc u rts n o c -e Dn o itilo m e d tro p s n a rT g n is s e c o rp e ts a W la s o p s iD -e s u e R-y re v o c e R-g n ilc y c e Rla itn e to p
A1 A2 A3 A4 A5 B1 B2 B3 B4 B5 B6 B7 C1 C2 C3 C4 D
X X X X X MND MND MNR MNR MNR MND MND X X X X X
RESULTS OF THE LCA - ENVIRONMENTAL IMPACT according to EN 15804+A2: 1 m² vinyl wallcoverings on cellulose fibre
base
Parameter Unit A1-A3 A4 A5 C1 C2 C3 C4 D
GWP-total kg CO 2 eq 3.9E-01 4.78E-02 3.35E-02 2.66E-05 2.11E-03 3.55E-01 0 -1.23E-01
GWP-fossil kg CO 2 eq 5.2E-01 4.77E-02 6.68E-03 2.66E-05 2.09E-03 2.54E-01 0 -1.23E-01
GWP-biogenic kg CO 2 eq -1.28E-01 0 2.68E-02 0 0 1.01E-01 0 0
GWP-luluc kg CO 2 eq -2.29E-03 9.45E-05 2.07E-06 8.89E-09 1.92E-05 1.69E-05 0 -7.83E-06
ODP kg CFC11 eq 1.72E-09 3.98E-15 3.82E-15 1.62E-16 2.7E-16 1.75E-13 0 -9.29E-13
AP mol H+ eq 1.39E-03 2.35E-04 1.02E-05 6.73E-08 1.74E-05 9.32E-05 0 -1.5E-04
EP-freshwater kg P eq 2.38E-05 4.32E-08 1.91E-09 2.34E-09 7.59E-09 5.6E-08 0 -1.92E-07
EP-marine kg N eq 4.27E-04 1.07E-04 3.83E-06 2.36E-08 8.66E-06 3.12E-05 0 -4.42E-05
EP-terrestrial mol N eq 4.36E-03 1.17E-03 4.78E-05 1.63E-07 9.56E-05 4.12E-04 0 -4.73E-04
kg NMVOC
POCP 1.26E-03 2.72E-04 9.53E-06 4.41E-08 1.64E-05 8.52E-05 0 -1.23E-04
eq
ADPE kg Sb eq 9.66E-08 1.05E-09 4.82E-11 1.53E-12 1.37E-10 1.54E-09 0 -8.55E-09
ADPF MJ 1.04E+01 6.45E-01 1.25E-02 4.75E-04 2.83E-02 3.8E-01 0 -2.24E+00
m3 world eq
WDP 3.05E-01 1.83E-04 4.1E-03 8.59E-03 2.51E-05 4.1E-02 0 -1.13E-02
deprived
GWP = Global warming potential; ODP = Depletion potential of the stratospheric ozone layer; AP = Acidification potential of land and water; EP =
Eutrophication potential; POCP = Formation potential of tropospheric ozone photochemical oxidants; ADPE = Abiotic depletion potential for non-fossil
resources; ADPF = Abiotic depletion potential for fossil resources; WDP = Water (user) deprivation potential)
RESULTS OF THE LCA - INDICATORS TO DESCRIBE RESOURCE USE according to EN 15804+A2: 1 m² vinyl wallcoverings on
cellulose fibre base
Parameter Unit A1-A3 A4 A5 C1 C2 C3 C4 D
PERE MJ 2.41E+00 1.21E-02 3.81E-01 9.67E-05 2.06E-03 1.25E+00 0 -6.34E-01
PERM MJ 1.53E+00 0 -3.79E-01 0 0 -1.15E+00 0 0
PERT MJ 3.94E+00 1.21E-02 2.57E-03 9.67E-05 2.06E-03 9.5E-02 0 -6.34E-01
PENRE MJ 7.12E+00 6.46E-01 9.78E-02 4.75E-04 2.84E-02 3.57E+00 0 -2.24E+00
PENRM MJ 3.28E+00 0 -8.52E-02 0 0 -3.19E+00 0 0
PENRT MJ 1.04E+01 6.46E-01 1.26E-02 4.75E-04 2.84E-02 3.8E-01 0 -2.24E+00
SM kg 2.18E-02 0 0 0 0 0 0 0
RSF MJ 0 0 0 0 0 0 0 0
NRSF MJ 0 0 0 0 0 0 0 0
FW m3 7.59E-03 1.37E-05 9.67E-05 2E-04 2.26E-06 9.98E-04 0 -5.14E-04
PERE = Use of renewable primary energy excluding renewable primary energy resources used as raw materials; PERM = Use of renewable primary
energy resources used as raw materials; PERT = Total use of renewable primary energy resources; PENRE = Use of non-renewable primary energy
excluding non-renewable primary energy resources used as raw materials; PENRM = Use of non-renewable primary energy resources used as raw
materials; PENRT = Total use of non-renewable primary energy resources; SM = Use of secondary material; RSF = Use of renewable secondary fuels;
NRSF = Use of non-renewable secondary fuels; FW = Use of net fresh water
RESULTS OF THE LCA – WASTE CATEGORIES AND OUTPUT FLOWS according to EN 15804+A2:
1 m² vinyl wallcoverings on cellulose fibre base
Parameter Unit A1-A3 A4 A5 C1 C2 C3 C4 D
HWD kg 1.37E-05 1.36E-12 3.09E-13 1.35E-14 8.79E-14 2.48E-12 0 -1.27E-10
NHWD kg 4.06E-02 6.72E-05 9.22E-04 6.08E-05 4.33E-06 9.34E-02 0 -1.09E-03
6 Environmental Product Declaration - IGI - The Global Wallcoverings Association - Vinyl wallcoverings on cellulose fibre base
RWD kg 1.08E-04 8.26E-07 5.28E-07 1.9E-08 5.31E-08 1.36E-05 0 -1.68E-04
CRU kg 0 0 0 0 0 0 0 0
MFR kg 0 0 0 0 0 0 0 0
MER kg 3.29E-02 0 2.22E-02 0 0 2.01E-01 0 0
EEE MJ 7.58E-02 0 0 0 0 0 0 5.6E-01
EET MJ 1.39E-01 0 0 0 0 0 0 1.07E+00
HWD = Hazardous waste disposed; NHWD = Non-hazardous waste disposed; RWD = Radioactive waste disposed; CRU = Components for re-use;
MFR = Materials for recycling; MER = Materials for energy recovery; EEE = Exported electrical energy; EET = Exported thermal energy
RESULTS OF THE LCA – additional impact categories according to EN 15804+A2-optional:
1 m² vinyl wallcoverings on cellulose fibre base
Parameter Unit A1-A3 A4 A5 C1 C2 C3 C4 D
Disease
PM 1.72E-08 9.79E-10 5.87E-11 1.08E-12 1.24E-10 1.3E-09 0 -1.27E-09
incidence
IR kBq U235 eq 1.75E-01 1.19E-04 8.38E-05 2.91E-06 7.93E-06 1.83E-03 0 -2.8E-02
ETP-fw CTUe 9.22E+00 4.53E-01 6.55E-03 9.77E-04 2.01E-02 2.21E-01 0 -4.78E-01
HTP-c CTUh 7.12E-10 8.53E-12 3.18E-13 1.86E-14 4.14E-13 1.01E-11 0 -2.46E-11
HTP-nc CTUh 6.72E-08 4.77E-10 1.35E-11 1.74E-12 2.51E-11 8.78E-10 0 -7.71E-10
SQP SQP 6.01E+00 5.92E-02 4.02E-03 7.06E-05 1.18E-02 8.89E-02 0 -4.17E-01
PM = Potential incidence of disease due to PM emissions; IR = Potential Human exposure efficiency relative to U235; ETP-fw = Potential comparative
Toxic Unit for ecosystems; HTP-c = Potential comparative Toxic Unit for humans (cancerogenic); HTP-nc = Potential comparative Toxic Unit for humans
(not cancerogenic); SQP = Potential soil quality index
Disclaimer 1 – for the indicator “Potential Human exposure efficiency relative to U235”. This impact category deals mainly with the
eventual impact of low-dose ionizing radiation on human health of the nuclear fuel cycle. It does not consider effects due to possible
nuclear accidents, occupational exposure or radioactive waste disposal in underground facilities. Potential ionizing radiation from the
soil, radon and from some construction materials is also not measured by this indicator.
Disclaimer 2 – for the indicators “abiotic depletion potential for non-fossil resources”, “abiotic depletion potential for fossil resources”,
“water (user) deprivation potential, deprivation-weighted water consumption”, “potential comparative toxic unit for ecosystems”,
“potential comparative toxic unit for humans – cancerogenic”, “Potential comparative toxic unit for humans - not cancerogenic”,
“potential soil quality index”. The results of this environmental impact indicator shall be used with care as the uncertainties on these
results are high as there is limited experience with the indicator.
This EPD was created using a software tool.
6. LCA: Interpretation
7 Environmental Product Declaration - IGI - The Global Wallcoverings Association - Vinyl wallcoverings on cellulose fibre base
carbon dioxide contained in the paper is treated first as a credit;
The production stage (module A1-A3) clearly dominates the after incineration in a waste-to-energy facility, it is treated as a
LCA results. The loads caused by the disposal stage (modules load (C3). Moreover, paper production has a relatively large
C3 and C4) become noticeable, especially as the biogenic influence on the acidification potential (AP), the eutrophication
carbon leaves the product system, reflected in the total and potential (EP), the ozone depletion (ODP), and the Potential for
biogenic global warming potential. Transports play a the formation of tropospheric ozone (POCP).
subordinate yet not insignificant role. The main environmental Transport processes also affect GWP-fossil, AP, EP, POCP, and
impacts are in all categories located in module A1-A3. For ADPF. The main reason is the combustion of fuels.
GWP-fossil and ADPF the highest precursor of impact is the The waste treatment in module C3 has a high participation in
use of PVC plastisol for vinyl coating. The use of thermal the GWP-fossil impact due to the incineration of PVC plastisol
energy for general production and heating/drying processes in at End-of-Life.
A3 is the second-highest precursor in both categories. The
production of paper and the use of electricity for production Range of the results
share the third place in the highest sources of GWP-fossil and The individual results of the participating companies
ADPF. differ from the average results in the present environmental
The highest source of environmental impact in most categories product declaration. Regarding GWP, the results may be 170%
is the production of PVC plastisol, not only because it higher or 32% lower than the average for this EPD.
constitutes 31% of the product mass; but because of the The main reason for the deviations is differences in the
energy-intensive production of PVC itself. grammage of the individual wallcoverings. In addition, there are
The production of new and recycled paper has a noticeable different materials used as well as varying heat and electricity
effect. It has a relatively high share of the greenhouse potential consumptions depending on the manufacturer.
due to energy demands. In the GWP category, the biogenic
7. Requisite evidence
Members of the The Global Wallcoverings Association have the • The wallcoverings meet the requirements of test
following certificates: standard ISO 16000.
• Optional compliance with German RAL-GZ 479.
• The declared products comply with EN 15102.
• Optional compliance with USA Wallcovering Association
• According to the (emission) test chamber assessment
W-101 (2013) paragraph 8.1 when tested by California
which follows the French measurement method Arrêté
Specification Section 01350 to criteria CDPH/EHLB
du 19/04/11 the wallcoverings meet the requirements of
Standard Method V1.1 (2010).
the test standard ISO 16000.
The certificates and classifications for the various wallcoverings
• Optional according to the chamber test which follows
can be obtained from the respective manufacturers.
the German AgBB (Committee for health-related
evaluation of building products) regulations
8. References
Standards and Norms Construction Product Regulation EU
Arrêté du 19/04/11 EN 12149:1997
Order of 19 April 2011 relating to the labeling of construction Wallcoverings in roll form - Determination of migration of heavy
products or wall or floor coverings and paints and varnishes on metals and certain other elements, of vinyl chloride monomer
their emissions of volatile pollutants and of formaldehyde release.
ASTM E 84 EN 12956:1999
ASTM E 84:2016: Standard Test Method for Surface Burning Wallcoverings in roll form - Determination of dimensions,
Characteristics of Building Materials straightness, spongeability and washability.
ASTM F 793 EN 13501-1:2018
ASTM F793 / F793M-15, Standard Classification of Wall Fire classification of construction products and building
Coverings by Use Characteristics, ASTM International, West elements - Part 1: Classification using data from reaction to fire
Conshohocken, PA, 2015 Tests.
ASTM F1141 - 93 EN 15102:2007+A1:2011
ASTM F1141-93(2009), Standard Specification for Decorative wallcoverings - Roll and panel form.
Wallcovering, ASTM International, West Conshohocken, PA,
2009 EN 233:2016
Wallcoverings in roll form - Specification for finished wallpapers,
BNB wall vinyls and plastics wallcoverings.
Lifetimes of components for life cycle analyses according to the
Bewertungssystem Nachhaltiges Bauen, 2011. EN 234:2019
Wallcoverings in roll form – Specification for wallcoverings for
CDPH/EHLB subsequent decoration
Standard method for measuring and evaluating chemical
emissions from indoor sources using environmental chambers, EN 235:2001
Version 1.1 Wallcoverings - Vocabulary and Symbols.
CPR EN 259-1:2001
8 Environmental Product Declaration - IGI - The Global Wallcoverings Association - Vinyl wallcoverings on cellulose fibre base
Wallcoverings in roll form - Heavy duty wallcoverings - Part 1: Regulation (EU) No 305/2011
Specifications. of the European Parliament and of the Council of 9 March 2011
laying down harmonised conditions for the marketing of
EN ISO 105-B02 construction products and repealing Council Directive
Textiles - Tests for colour fastness - Part B02: Colour fastness 89/106/EEC Text with EEA relevance. Current consolidated
to artificial light: Xenon arc fading lamp test (ISO 105- version: 16/07/2021
B02:2014).
WA-101
EN ISO 14025:2006 WA Quality Standard for Polymer Coated Fabric Wallcovering
Environmental labels and declarations — Type III
environmental declarations — Principles and procedures; 2009-
11. Further documentation
EN ISO 14044:2006 Ecoinvent
Environmental management - Life cycle assessment - Database for Life Cycle Assessment, version 3.6. Swiss Center
Requirements and guidelines (ISO 14044:2006). for Life Cycle Inventories, St. Gallen, 2023.
EN ISO 16000:2006 European Commission
Indoor air - Part 3: Determination of formaldehyde and other List of substances banned for use in cosmetic products. CMR
carbonyl compounds in indoor air and test chamber air - Active substances of category 1A, 1B or 2 under Commission
sampling method. Regulation (EC) No 790/2009. 01/12/2010. Updated
Indoor air - Part 6: Determination of volatile organic compounds 01/07/2015.
in indoor and test chamber air by active sampling on Tenax
TA® sorbent, thermal desorption and gas chromatography European Parliament
using MS or MS-FID. Regulation (EU) no 528/2012 of the European Parliament and
Indoor air - Part 9: Determination of the emission of volatile of the council of 22 may 2012 concerning the making available
organic compounds from building products and furnishing - on the market and use of biocidal products.
Emission test chamber method.
Indoor air - Part 11: Determination of the emission of volatile European Waste Catalogue (EWC)
organic compounds from building products and furnishing - European Waste Catalogue / Ordinance on European List of
Sampling, storage of samples and preparation of test Wastes
specimens.
EU-JRC
ISO 14001:2015 EN 15804 reference package. Flows, Methods,
Environmental management systems - Requirements with Characterisation Factors, Unit Groups and Flow Properties
guidance for use. based on EF Reference Package 3.0.
EN 15804 German AgBB
EN 15804:2012+A2:2019+AC:2021, Sustainability of Committee for health-related evaluation of building products.
construction works — Environmental Product Declarations — Umweltbundesamt Deutschlands.
Core rules for the product category of construction products.
Institut Bauen und Umwelt e. V.
ISO 50001:2011 Product Category Rules for Building-Related Products and
Energy management systems - Requirements with guidance for Services – PCR-A: Part A+A2: Calculation Rules for the Life
use. Cycle Assessment and Requirements on the Project Report
according to EN 15804+A2:2019, version: 1.3 from 31/08/2022.
SVHC
Candidate List of substances of very high concern for Institut Bauen und Umwelt e. V.
Authorisation (SVHC) PCR Guidance-Texts for Building-Related Products and
Published in accordance with Article 59(10) of the REACH Services - Part B: Requirements on the EPD for Wallcoverings.
Regulation. European chemicals agency (ECHA). Version: 8 from 01/08/2021.
RAL-GZ 479 LCA for Experts (GaBi)
Wallpapers - Quality assurance LCA for Experts 10.7.0.183: Software System and Database for
Life Cycle Engineering. 1992-2023. Sphera Solutions GmbH
9 Environmental Product Declaration - IGI - The Global Wallcoverings Association - Vinyl wallcoverings on cellulose fibre base
Publisher
Institut Bauen und Umwelt e.V. +49 (0)30 3087748- 0
Hegelplatz 1 info@ibu-epd.com
10117 Berlin www.ibu-epd.com
Germany
Programme holder
Institut Bauen und Umwelt e.V. +49 (0)30 3087748- 0
Hegelplatz 1 info@ibu-epd.com
10117 Berlin www.ibu-epd.com
Germany
Author of the Life Cycle Assessment
brands & values GmbH +49 421 70 90 84 33
Altenwall 14 info@brandsandvalues.com
28195 Bremen www.brandsandvalues.com
Germany
Owner of the Declaration
IGI - The Global Wallcoverings Association +32 (0) 2 720 00 09
Chaussée de Louvain 426 info@igiwallcoverings.org
1380 LASNE www.igiwallcoverings.org
Belgium
10 Environmental Product Declaration - IGI - The Global Wallcoverings Association - Vinyl wallcoverings on cellulose fibre base
