ENVIRONMENTAL PRODUCT DECLARATION
as per ISO 14025 and EN 15804+A2
Owner of the Declaration ARGE – The European Federation of Locks and Building Hardware Manufacturers
Publisher Institut Bauen und Umwelt e.V. (IBU)
Programme holder Institut Bauen und Umwelt e.V. (IBU)
Declaration number EPD-ARG-20230544-IBG1-EN
Issue date 02.04.2024
Valid to 01.04.2029
Padlocks
ARGE – The European Federation of Locks
and Building Hardware Manufacturers
This EPD is valid only for products supplied by an ARGE EPD licence holder.
www.ibu-epd.com | https://epd-online.com
1. General Information
ARGE – The European Federation of Locks Padlocks
and Building Hardware Manufacturers
Programme holder Owner of the declaration
IBU – Institut Bauen und Umwelt e.V. ARGE – The European Federation of Locks and Building Hardware
Hegelplatz 1 Manufacturers
10117 Berlin Offerstraße 12
Germany 42551 Velbert
Germany
Declaration number Declared product / declared unit
EPD-ARG-20230544-IBG1-EN 1 kg of padlock
This declaration is based on the product category rules: Scope:
Building Hardware products, 01.08.2021 This ARGE EPD covers padlocks and padlock fittings operated by means
(PCR checked and approved by the SVR) of a key. They are used for securing buildings, both outside and inside. The
reference product used to calculate the impact this product group has on
the environment is a padlock composed primarily of steel, Zamak and
Issue date brass. This product is the only one assessed for this EPD and serves as
reference to cover all products within this family. This product has been
02.04.2024
determined in accordance with ARGE and the market share as the most
representative product of the family.
The owner of the declaration shall be liable for the underlying information
Valid to
and evidence; the IBU shall not be liable with respect to manufacturer
01.04.2029 information, life cycle assessment data and evidences.
The EPD was created according to the specifications of EN 15804+A2. In
the following, the standard will be simplified as EN 15804.
Verification
The standard EN 15804 serves as the core PCR
Independent verification of the declaration and data according to ISO
14025:2011
internally X externally
Dipl.-Ing. Hans Peters
(Chairman of Institut Bauen und Umwelt e.V.)
Florian Pronold Dr. Matthew Fishwick,
(Managing Director Institut Bauen und Umwelt e.V.) (Independent verifier)
1 Environmental Product Declaration - ARGE – The European Federation of Locks and Building Hardware Manufacturers - Padlocks
2. Product
the ring-opening polymerisation of caprolactam. Components
2.1 Product description/Product definition
made of Nylon 6 are formed by injection moulding or other
This ARGE EPD covers external locking devices, including the thermal forming processes.
corresponding fittings, used to secure doors and gates to
frames. For the application and use the respective national 1) This product/article/at least one partial article contains
provisions at the place of use apply. substances listed in the ECHA candidate list (date: 14.06.2023)
exceeding 0.1 percentage by mass: Certain components may
2.2 Application
contain small amounts of lead (CAS no. 7439-92-1) as an
Padlocks are used as a stand-alone product to secure doors alloying element.
and gates without the need for a locking mechanism integrated
into the door or gate. 2) This product/article/at least one partial article contains other
cancerogenic, mutagenic, reprotoxic (CMR) substances in
2.3 Technical Data
categories 1A or 1B which are not on the ECHA candidate list,
Ideally, products comply with a suitable technical specification.
exceeding 0.1 percentage by mass: no.
EN 12320:2021, Building hardware - Padlocks and padlock
fittings - Requirements and test methods is an example of such
3) Biocide products were added to this construction product or it
a specification and some products will comply with this. The
has been treated with biocide products (this then concerns a
relevant grading structure is shown in the following table:
treated product as defined by the (EU) Ordinance on Biocide
Name Value Unit
Products No. 528/2012): no.
Category of use 1 Grade
2.6 Manufacture
Durability 0,1 Grade
The manufacture of a padlock usually follows a 3-step process:
Corrosion resistance 1 - 6 Grade
Safety 1 - 6 Grade 1. Manufacture of the components: this step may include
surface treatment in the factory or by external
Performance data of the product with respect to its
contractors.
characteristics in accordance with the relevant technical
2. Pre-assembly of modules (in the factory).
provision (no CE-marking).
3. Final assembly (in the factory).
2.4 Delivery status
2.7 Environment and health during manufacturing
The products are sold by unit. Deliveries of individual items are Regular measurements of air quality and noise levels are
possible but are an exception. Standard deliveries comprise a carried out by the manufacturers, the ARGE member
larger quantity of padlocks, as they are marketed as "B2B"
companies. The results shall be within the mandatory safety
products and not to end-users.
levels. In areas where employees are exposed to chemical
products, the required protective clothing and technical
2.5 Base materials/Ancillary materials
protective devices shall be provided. Regular health checks are
Composition of product analysed for this EPD:
mandatory for employees in production facilities.
The values given in the table below are for the product 2.8 Product processing/Installation
analysed for this EPD.
The installation of the product may vary depending on the type
Name Value Unit of door or gate and the specific situation, but the products shall
Steel 88.17 % not require energy consumption for installation.
Zamak 5.97 %
2.9 Packaging
Brass 3.05 %
Normally, each individual product is packed in paper or
Stainless steel 2.13 % cardboard. These individual products are then packed in a
Nylon 6 0.64 % cardboard box and stacked on wooden pallets for transport to
the customer.
Steel is produced by combining iron with carbon as well as
Waste from product packaging is collected separately for waste
other elements depending on the desired characteristics.
disposal (including recycling).
Components made of steel are formed by different types of
mechanical processing. 2.10 Condition of use
Once installed, products shall require no servicing during their
Zamak is an alloy with a base metal of zinc and alloying
expected service lives. There shall be no consumption of water
elements of aluminium, magnesium, and copper. Components
or energy linked to their use, and they shall not cause any
made of Zamak are die-cast.
emissions.
Brass is an alloy of zinc and copper. Components made of 2.11 Environment and health during use
brass are made by extrusion, forging, die-casting or other types No environmental damage or health risks are to be expected
of mechanical processing. during normal conditions of use.
Stainless steel is produced by combining iron with chromium 2.12 Reference service life
as well as other elements depending on the desired The reference service life is 30 years under normal working
characteristics. Components made of steel are formed by conditions. This corresponds to passing a mechanical
stamping or other types of mechanical processing. endurance test of 10.000 cycles as specified in the EN 12320.
The reference service life is dependent on the actual frequency
Nylon 6 is a polymer, in particular polyamide. It is formed by of use and environmental conditions. It is required that
2 Environmental Product Declaration - ARGE – The European Federation of Locks and Building Hardware Manufacturers - Padlocks
installation, as well as maintenance of the product, must be the environment.
done in line with instructions provided by the manufacturer.
2.14 Re-use phase
2.13 Extraordinary effects Removal of padlocks and their fittings (for re-use or recycling)
Fire shall have no adverse effect on the environment.
There are no fire resistance requirements in EN 12320. So, any
fire resistance requirements would be a voluntary declaration 2.15 Disposal
by the manufacturer. Padlocks and their fittings should be recycled wherever
possible, providing that there is no adverse effect on the
Water environment. The waste code in accordance with the European
The declared product is intended to be used on buildings under Waste Code is 17 04 07.
normal conditions (usually outdoors). It shall not emit
2.16 Further information
hazardous substances in the event of flooding.
Details of all types and variants can be found on the
manufacturers' websites. The respective website addresses are
Mechanical destruction
available at https://arge.org.
Mechanical destruction of the declared product shall not
materially alter its composition or have any adverse effect on
3. LCA: Calculation rules
attained the 'end-of-waste' state.
3.1 Declared Unit
• each type of waste is modelled as a transport to the
The declared unit for all products covered by ARGE EPD is 1 treatment site with a distance of 30 km. Parts sent for
kg (of product). Since individual products will rarely weigh recycling include electricity consumption (grinding) and
exactly 1 kg it is necessary to establish the exact weight of the a flow ('Materials for recycling, unspecified').
product and then use this as a correction factor to determine
the true values for 1 kg of product in the tables (Section 5). 3.3 Estimates and assumptions
The LCA data of the declared product have been calculated
Declared unit
using the production data of one ARGE member company. This
Name Value Unit
company has been chosen by ARGE as being representative
Declared unit 1 kg by means of its production processes and its market share. The
Mass of declared product 0.469 kg product is chosen to be as representative as possible.
Raw density 1 kg/m3
3.4 Cut-off criteria
The cut-off criteria considered are 1% of renewable and non-
renewable primary energy usage and 1% of the total mass of
3.2 System boundary
that unit process. The total neglected input flows per module
Type of the EPD: "cradle to gate with options, with modules C1 shall be a maximum of 5% of energy usage and mass.
– C4, and module D (A1-A3, C1-C3, D and additional
modules)" For this study, all input and output flows have been considered
at 100%, including raw materials as per the product
The analysis of the product life cycle includes the production composition provided by the manufacturer and packaging of
and transport of the raw materials, the manufacture of the raw materials as well as the final product. Energy and water
product and the packaging materials which are declared in consumptions have also been considered at 100% according to
modules A1-A3. the data provided.
Losses during production are considered as waste and are sent
for recycling. No recycling processes are taken into account With the approach chosen, no significant environmental
except for transport and electricity consumption for grinding the impacts are known to have been cut off.
metals. When recycled metals are used as raw material only
their transformation process is taken into account and not the 3.5 Background data
extraction of the raw material. For the life cycle modelling of the considered product, all
A4 module represents the transport of the finished padlock to relevant background datasets are taken from ecoinvent v3.8
the installation site. (system model: cut-off by classification).
There is nowaste associated with the installation of the product.
The A5 module therefore represents only the disposal of the 3.6 Data quality
product packaging. The objective of this evaluation is to evaluate the environmental
The End-of-Life (EoL) stages are also considered. The impacts generated by the products throughout their entire life
transportation to the EoL disposal site is taken into account in cycles. To this end, ISO 14040, ISO 14044 and EN 15804 have
module C2. Module C4 covers the disposal of the locks. Module been met regarding the quality of data on the following different
C3 covers the recycling of the individual elements according to criteria:
European averages, with the remaining waste divided between
incineration and landfill. Such a mixed scenario is declared due Time: The life cycle inventory data used come from:
to the complex material mix of the product and the dependency
• Data collected specifically for this study on the ARGE
of the EoL-route on the EoL-route of the product the padlock
member company's manufacturing site. Datasets are
has been integrated into.
based on 1-year averaged data (time period: January
In practice, the end of life has been modelled as follows:
2013 to December 2013 considered representative for
• when a material is sent for recycling, generic transport 2022).
and electric consumption of a shredder is taken into • In the absence of collected data, generic data from the
account (corresponding to the process 'Grinding, ecoinvent v3.8 database have been used. This is
metals'). Only then, is the material considered to have updated regularly and is representative of current
3 Environmental Product Declaration - ARGE – The European Federation of Locks and Building Hardware Manufacturers - Padlocks
processes (the entire database having been updated in lifespan: Europe
2021).
Geography: Data on the composition of products, process
3.9 Allocation
technologies, wastage, etc. come from production site of the
ARGE member company. Generic data on processing The products covered by this EPD are produced in numerous
processes come from the ecoinvent database, representative sites. The product assessed for the calculation of this EPD is
for European production processes. produced by one manufacturer on one site. All data were
provided by this manufacturer of the products per unit, and then
Technology: Material shaping technologies are based on divided by the mass of the product to give a value per kg of
European technology in the case of the use of generic data. product produced.
In this EPD, a representative product has been selected to
represent the product group, considering the most common The assumptions relating to the EoL of the product are
materialisation of the products covered in this product group. described in the section System Boundaries.
3.7 Period under review 3.10 Comparability
The data of the LCA is based on the annual production data of Basically, a comparison or an evaluation of EPD data is only
an ARGE member from 2013, considered representative for the possible if all the data sets to be compared were created
year 2022. according to EN 15804 and the building context, respectively
the product-specific characteristics of performance, are taken
3.8 Geographic Representativeness into account. ecoinvent v3.8 (system model: cut-off by
Land or region, in which the declared product system is classification) has been used as the background database.
manufactured, used or handled at the end of the product´s
4. LCA: Scenarios and additional technical information
It is assumed that a 16–32-ton truck is used to transport the
Characteristic product properties of biogenic carbon
product:
- Transport to shredding facility for metal recovery: 150 km
Information on the biogenic carbon content at factory gate - Transport to municipal waste incineration plant: 50 km
- Transport to landfill: 30 km
Note: 1 kg of biogenic carbon is equivalent to 44/12 kg of CO .
2
Name Value Unit
kg Reuse, recovery and/or recycling potentials (D), relevant
Biogenic carbon content in product 0
C scenario information
Biogenic carbon content in accompanying kg
0.0570
packaging C Module D contains the benefits and loads beyond the system
boundary related to the recycling of metals, which result from
the treatment of recycled materials from the point of end-of-
The following information is the basis of the declared modules
waste status to the point of substitution (as costs) and the
within the LCA in this EPD.
substitution of primary resources (as benefits).
Transport to the building site (A4)
Name Value Unit According to EN 16710, clause 6.4.3.3: 'In module D
substitution effects are calculated only for the resulting net
Litres of fuel 25.8 l/100km
output flow.
Transport distance 3500 km
Capacity utilisation (including empty runs) 36 % For building hardware, the following rules apply for the
quantification of net output flows:
Installation into the building (A5)
- all production scrap and cuttings leave modules A1-B3 as
Name Value Unit sorted scrap without allocated burdens from primary production;
Material loss 0.144 kg the corresponding amounts are declared as material for
recycling (MFR);
- net amounts of a metal leaving the product system are
Reference service life quantified as the material for recycling leaving modules A1-C4
Name Value Unit minus the input of secondary scrap (secondary material, SM) to
the product system;
Reference service life 30 a
- in the case of brass and zinc alloys, which are composed of
Test cycles over RSL (EN 12320) 10'000 cycles
two different constituting metals, no difference shall be made
between the input of secondary constituting metals (Cu and Zn;
End of life (C1-C4)
Cu and Sn) and its alloys (CuZn; CuSn).
Name Value Unit
Collected separately waste type (Mixed scenario) 1 kg Negative net output flows have not been considered in the
Recycling (Mixed scenario) 0.796 kg quantification of module D.
Energy recovery (Mixed scenario) 0.094 kg
It also includes the benefits and loads related to 'exported
Landfilling (Mixed scenario) 0.11 kg
energy electricity' and 'exported energy heat' resulting from the
Incineration (100% incineration scenario) Scenario
1 kg energy recovery from plastic wastes in a municipal waste
1
incineration plant as modelled in Modules A3, A5 and C4.
Landfilling (100% Landfill scenario) Scenario 2 1 kg
Recycling (100% recycling scenario) Scenario 3 1 kg
4 Environmental Product Declaration - ARGE – The European Federation of Locks and Building Hardware Manufacturers - Padlocks
5. LCA: Results
In Table 1 "Description of the system boundary", the declared modules are indicated with an "X"; all modules that are not declared
within the EPD but where additional data are available are indicated with "MND". Those data can also be used for building assessment
scenarios. The values are declared with three valid digits in exponential form.
The set of characterisation factors EF3.0 has been used for the life cycle assessment.
DESCRIPTION OF THE SYSTEM BOUNDARY (X = INCLUDED IN LCA; MND = MODULE OR INDICATOR NOT DECLARED; MNR
= MODULE NOT RELEVANT)
Benefits and
Construction loads beyond
Product stage Use stage End of life stage
process stage the system
boundaries
la ire wta am R y lp p u s tro p s n a rT g n iru tc a fu n a M tro p s nm ae o rh r
T
f te tis e h t o t e ta g y lb m e s s A e s U e c n a n e tn ia M ria p e R tn e m e c a lp e R tn e m h s ib ru fe R la n o ity ag rr ee pn Oe e s u la n o ita r re et pa Ow e s u n o itc u rts n eo Dc -n o itilo m e d tro p s n a rT g n is s ee tsc ao Wrp la s o p s iD e s u e R- y re v o c e R- g n ilc y c e R- la itn e to p
A1 A2 A3 A4 A5 B1 B2 B3 B4 B5 B6 B7 C1 C2 C3 C4 D
X X X X X MND MND MNR MNR MNR MND MND X X X X X
RESULTS OF THE LCA - ENVIRONMENTAL IMPACT according to EN 15804+A2: 1 kg of padlock
Parameter Unit A1-A3 A4 A5 C1 C2 C3 C4 D
GWP-total kg CO2 eq 5.14E+00 6.52E-01 2.32E-01 0 1.86E-02 4.48E-03 8.27E-03 -1.13E+00
GWP-fossil kg CO2 eq 5.34E+00 6.52E-01 2.33E-02 0 1.86E-02 4.46E-03 8.27E-03 -1.13E+00
GWP-biogenic kg CO2 eq -2.09E-01 0 2.09E-01 0 0 0 0 0
GWP-luluc kg CO2 eq 7.41E-03 2.61E-04 1.24E-06 0 7.45E-06 1.11E-05 2.1E-06 -9.95E-04
ODP kg CFC11 eq 3.42E-07 1.51E-07 6.91E-10 0 4.32E-09 2.26E-10 7.31E-10 -4.65E-08
AP mol H+ eq 4.19E-02 1.85E-03 1.72E-05 0 5.29E-05 2.3E-05 1.92E-05 -1.13E-02
EP-freshwater kg P eq 4.1E-04 4.65E-06 2.96E-08 0 1.33E-07 5.02E-07 4.1E-08 -7.16E-05
EP-marine kg N eq 6.69E-03 3.68E-04 6.11E-06 0 1.05E-05 2.95E-06 6.83E-06 -1.2E-03
EP-terrestrial mol N eq 6.49E-02 4.1E-03 6.6E-05 0 1.17E-04 3.41E-05 7.2E-05 -1.47E-02
kg NMVOC
POCP 2.08E-02 1.58E-03 1.85E-05 0 4.5E-05 9.32E-06 2.18E-05 -5.73E-03
eq
ADPE kg Sb eq 5.68E-04 2.31E-06 1.14E-08 0 6.6E-08 1.08E-08 8.49E-09 -2.34E-04
ADPF MJ 7.03E+01 9.89E+00 4.76E-02 0 2.82E-01 9.46E-02 5.34E-02 -1.07E+01
m3 world eq
WDP 1.93E+00 3.01E-02 3E-04 0 8.6E-04 1.06E-03 -5.78E-04 -2.82E-01
deprived
GWP = Global warming potential; ODP = Depletion potential of the stratospheric ozone layer; AP = Acidification potential of land and water; EP =
Eutrophication potential; POCP = Formation potential of tropospheric ozone photochemical oxidants; ADPE = Abiotic depletion potential for non-fossil
resources; ADPF = Abiotic depletion potential for fossil resources; WDP = Water (user) deprivation potential)
RESULTS OF THE LCA - INDICATORS TO DESCRIBE RESOURCE USE according to EN 15804+A2: 1 kg of padlock
Parameter Unit A1-A3 A4 A5 C1 C2 C3 C4 D
PERE MJ 1.05E+01 1.39E-01 -7.08E-01 0 3.97E-03 1.79E-02 8.67E-04 -1.21E+00
PERM MJ 1.78E+00 0 -2.15E-01 0 0 0 0 0
PERT MJ 1.23E+01 1.39E-01 -9.23E-01 0 3.97E-03 1.79E-02 8.67E-04 -1.21E+00
PENRE MJ 7.01E+01 9.89E+00 3.38E-01 0 2.83E-01 9.55E-02 1.33E-01 -1.07E+01
PENRM MJ 4.5E-01 0 -2.9E-01 0 0 0 -7.99E-02 0
PENRT MJ 7.06E+01 9.89E+00 4.76E-02 0 2.83E-01 9.55E-02 5.34E-02 -1.07E+01
SM kg 3.56E-01 0 0 0 0 0 0 0
RSF MJ 0 0 0 0 0 0 0 0
NRSF MJ 0 0 0 0 0 0 0 0
FW m3 6.38E-02 1.05E-03 5.19E-05 0 3E-05 6.09E-05 1.31E-04 -7.13E-03
PERE = Use of renewable primary energy excluding renewable primary energy resources used as raw materials; PERM = Use of renewable primary
energy resources used as raw materials; PERT = Total use of renewable primary energy resources; PENRE = Use of non-renewable primary energy
excluding non-renewable primary energy resources used as raw materials; PENRM = Use of non-renewable primary energy resources used as raw
materials; PENRT = Total use of non-renewable primary energy resources; SM = Use of secondary material; RSF = Use of renewable secondary fuels;
NRSF = Use of non-renewable secondary fuels; FW = Use of net fresh water
RESULTS OF THE LCA – WASTE CATEGORIES AND OUTPUT FLOWS according to EN 15804+A2:
1 kg of padlock
Parameter Unit A1-A3 A4 A5 C1 C2 C3 C4 D
HWD kg 3.15E-04 2.58E-05 2.15E-07 0 7.37E-07 3.35E-08 1.03E-07 -1.18E-04
NHWD kg 2.41E+00 5.2E-01 3.19E-03 0 1.49E-02 3.56E-04 2.29E-01 -5.11E-01
RWD kg 5.8E-04 1.43E-04 6.17E-07 0 4.09E-06 1.27E-06 6.82E-07 -2.3E-05
CRU kg 0 0 0 0 0 0 0 0
MFR kg 1.99E-01 0 9.3E-02 0 0 6.68E-01 0 0
MER kg 0 0 0 0 0 0 0 0
5 Environmental Product Declaration - ARGE – The European Federation of Locks and Building Hardware Manufacturers - Padlocks
EEE MJ 5.74E-04 0 3.71E-02 0 0 0 3.39E-03 0
EET MJ 3.8E-03 0 2.45E-01 0 0 0 2.24E-02 0
HWD = Hazardous waste disposed; NHWD = Non-hazardous waste disposed; RWD = Radioactive waste disposed; CRU = Components for re-use;
MFR = Materials for recycling; MER = Materials for energy recovery; EEE = Exported electrical energy; EET = Exported thermal energy
RESULTS OF THE LCA – additional impact categories according to EN 15804+A2-optional:
1 kg of padlock
Parameter Unit A1-A3 A4 A5 C1 C2 C3 C4 D
Disease
PM 3.5E-07 5.24E-08 3E-10 0 1.5E-09 6.14E-11 5.66E-10 -7.26E-08
incidence
IR kBq U235 eq 3.46E-01 4.29E-02 1.88E-04 0 1.23E-03 8.62E-04 2.05E-04 -1.07E-02
ETP-fw CTUe 3.16E+02 7.76E+00 4.49E-02 0 2.22E-01 4.76E-02 1.17E-01 -9.28E+01
HTP-c CTUh 2.63E-08 2.5E-10 3.37E-12 0 7.13E-12 1.27E-12 6.5E-12 -1.43E-10
HTP-nc CTUh 4.02E-07 7.84E-09 1.37E-10 0 2.24E-10 4.13E-11 5.96E-11 -8.06E-09
SQP SQP 5.9E+01 6.89E+00 3.03E-02 0 1.97E-01 1.45E-02 9.09E-02 -5.78E+00
PM = Potential incidence of disease due to PM emissions; IR = Potential Human exposure efficiency relative to U235; ETP-fw = Potential comparative
Toxic Unit for ecosystems; HTP-c = Potential comparative Toxic Unit for humans (cancerogenic); HTP-nc = Potential comparative Toxic Unit for humans
(not cancerogenic); SQP = Potential soil quality index
Disclaimer 1 –
for the indicator 'Potential Human exposure efficiency relative to U235'. This impact category deals mainly with the eventual impact of
low-dose ionizing radiation on human health of the nuclear fuel cycle. It does not consider effects due to possible nuclear accidents,
occupational exposure or radioactive waste disposal in underground facilities. Potential ionizing radiation from the soil, radon and from
some construction materials is also not measured by this indicator.
Disclaimer 2 –
for the indicators 'abiotic depletion potential for non-fossil resources', 'abiotic depletion potential for fossil resources', 'water (user)
deprivation potential, deprivation-weighted water consumption', 'potential comparative toxic unit for ecosystems', 'potential comparative
toxic unit for humans – cancerogenic', 'Potential comparative toxic unit for humans - not cancerogenic', 'potential soil quality index'. The
results of this environmental impact indicator shall be used with care as the uncertainties on these results are high as there is limited
experience with the indicator.
6. LCA: Interpretation
Figure 1 illustrates the relative contributions of the different
modules along the life cycle of the declared products.
significant.
Figure 1: Environmental impacts of padlocks along its life
cycle Benefits and burdens beyond the system boundary (module D)
are in the order of 10 % to 30 % of the impacts over the product
The largest part of environmental impacts is caused during life cycle (modules A1-A3) and relate basically to the recycling
production (modules A1-A3); comparably small impacts are of metals.
caused during the transport of the product to the construction In this EPD, a representative product has been selected to
site (via the manufacturer of the product, which the padlock has represent the product group, considering the most common
been integrated into). materialisation of the products covered in this product group.
This has been done based on the knowledge of ARGE
All the other modules related to the product life cycle are not members on the composition of the declared products. In in-
6 Environmental Product Declaration - ARGE – The European Federation of Locks and Building Hardware Manufacturers - Padlocks
depth analysis of variability has not been conducted for this product group.
7. Requisite evidence
No testing results are required by the PCR part B.
8. References
Product category rules of IBU 14044:2006); German and English versions EN ISO
14044:2006.
IBU (2021)
IBU (2021): General Instructions for the EPD Programme of the EN 12320
Institut Bauen und Umwelt e.V. (General Instructions for the EN 12320:2021, Building hardware - Padlocks and padlock
IBU EPD Programme). Version 2.0, Institut Bauen und Umwelt, fittings - Requirements and test methods.
Berlin.
ISO 15686
IBU (2021) ISO 15686:1, -2, -7 and -8. Service life planning (various parts).
IBU (2021): PCR Part A: Calculation rules for the life cycle
assessment and requirements on the project report according ECHA candidate list
to EN 15804+A2. Version 1.3., Institut Bauen und Umwelt, Candidate List of substances of very high concern for
Berlin. Authorisation, published in accordance with Article 59(10) of the
REACH Regulation. European Chemicals Agency, Brussels.
IBU (2023)
IBU (2023): ): PCR Part B: Requirements on the EPD for Ordinance on Biocide Products No. 528/2012
building hardware products. Version 2023/04, Institut Bauen REGULATION (EU) No 528/2012 OF THE EUROPEAN
und Umwelt, Berlin. PARLIAMENT AND OF THE COUNCIL of 22 May 2012
concerning the making available on the market and use of
Standards and legal documents biocidal products.
EN 15804 European List of Waste
EN 15804:2012+A2:2019+AC:2021, Sustainability of Commission Decision of 3 May 2000 replacing Decision
construction works - Environmental product declarations - Core 94/3/EC establishing a list of wastes pursuant to Article 1(a) of
rules for the product category of construction products. Council Directive 75/442/EEC on waste and Council Decision
94/904/EC establishing a list of hazardous waste pursuant to
EN 17610 Article 1(4) of Council Directive 91/689/EEC on hazardous
EN 17610:2022, Building hardware - Environmental product waste (notified under document number C(2000) 1147).
declarations - Product category rules complementary to EN
15804 for building hardware. Additional references
ISO 14025 BBSR 2017
ISO 14025:2006-07, Environmental labels and declarations - BBSR (2017): Nutzungsdauer von Bauteilen in
Type III Environmental declarations - Principles and Lebenszyklusanalysen nach Bewertungssystem Nachhaltiges
procedures. Bauen (BNB). Version vom 24.10.2017, Bundesinstitut für Bau-,
Stadt- und Raumforschung, Berlin.
ISO 14044
EN ISO 14044:2006-07, Environmental management - Life ecoinvent v3.8
cycle assessment - Requirements and guidance (ISO http://www.ecoinvent.org
7 Environmental Product Declaration - ARGE – The European Federation of Locks and Building Hardware Manufacturers - Padlocks
Publisher
Institut Bauen und Umwelt e.V. +49 (0)30 3087748- 0
Hegelplatz 1 info@ibu-epd.com
10117 Berlin www.ibu-epd.com
Germany
Programme holder
Institut Bauen und Umwelt e.V. +49 (0)30 3087748- 0
Hegelplatz 1 info@ibu-epd.com
10117 Berlin www.ibu-epd.com
Germany
Author of the Life Cycle Assessment
Dr. Frank Werner - Umwelt & Entwicklung + 41 (0)44 241 39 06
Kammelenbergstrasse 30 frank@frankwerner.ch
9011 St. Gallen http://www.frankwerner.ch/
Switzerland
Owner of the Declaration
ARGE – The European Federation of Locks and +49 (0)2051 9506 15
Building Hardware Manufacturers mail@arge.org
Offerstraße 12 www.arge.org
42551 Velbert
Germany
8 Environmental Product Declaration - ARGE – The European Federation of Locks and Building Hardware Manufacturers - Padlocks
