Environmental product declaration
In accordance with ISO 14025 and EN 15804 +A2
weber WX Waterproofing membrane (weber WX Vedeneriste)
Owner of the declaration: Program operator:
Saint-Gobain Finland Oy The Norwegian EPD Foundation
Declared unit: Declaration number:
1 kg weber WX Waterproofing membrane (weber WX
Vedeneriste) NEPD-3969-3004-EN
This declaration is based on Product Category Rules: Registration number:
CEN Standard EN 15804:2012+A2:2019 serves as core PCR
NPCR 009:2018 Part B for Technical - Chemical products in the NEPD-3969-3004-EN
building and construction industry
Issue date: 02.12.2022
Valid to: 02.12.2027
The Norwegian EPD Foundation
EPD Software:
LCA.no EPD generator
System ID:
54574
1 / 12
General information
Product Owner of the declaration:
weber WX Waterproofing membrane (weber WX Vedeneriste) Saint-Gobain Finland Oy
Contact person: Anne Kaiser
Phone: +358400289933
e-mail: anne.kaiser@saint-gobain.com
Program operator: Manufacturer:
Post Box 5250 Majorstuen, 0303 Oslo, Norway Saint-Gobain Finland Oy
The Norwegian EPD Foundation P.O. Box 70 , Fi-00381 Helsinki
Phone: +47 23 08 80 00 Finland
web: post@epd-norge.no
Declaration number: Place of production:
NEPD-3969-3004-EN Scanspac Sala
Norrängsgatan 35 , 73338 Sala
Sweden
Management system:
This declaration is based on Product Category Rules: ISO 9001:2015, ISO 14001:2015 and OHSAS 18001:2007
CEN Standard EN 15804:2012+A2:2019 serves as core PCR
NPCR 009:2018 Part B for Technical - Chemical products in the building and
construction industry
Organisation no:
Statement of liability: FI09515553
The owner of the declaration shall be liable for the underlying information and
evidence. EPD Norway shall not be liable with respect t​o manufacturer
information, life cycle assessment data and evidences.
Issue date: 02.12.2022
Declared unit:
1 kg weber WX Waterproofing membrane (weber WX Vedeneriste)
Declared unit with option: Valid to: 02.12.2027
A1-A3,A4,A5,C1,C2,C3,C4,D
Functional unit: Year of study:
Functional unit is not used because use stage is not considered. 2021
General information on verification of EPD from EPD tools: Comparability:
Independent verification of data, other environmental information and the EPD of construction products may not be comparable if they not comply with
declaration according to ISO 14025:2010, § 8.1.3 and § 8.1.4. Individualthird party EN 15804 and seen in a building context.
verification of each EPD is not required when the EPD tool is i) integrated into the
company's environmental management system, ii) the procedures for use of the
EPD tool are approved by EPDNorway, and iii)the proccess is reviewed annualy.
See Appendix G of EPD-Norway's General Programme Instructions for further
information on EPD tools.
Verification of EPD tool: Development and verification of EPD:
The declaration is created using EPD tool lca.tools ver EPD2022.03, developed by
Independent third party verification of the EPD tool, background data and test-
EPD in accordance with EPDNorway's procedures and guidelines for verification LCA.no. The EPD tool is integrated in the company's management system, and
and approval of EPD tools. has been approved by EPD Norway.
Third party verifier: Developer of EPD:
Päivi Pesu
Reviewer of company-specific input data and EPD:
Anne Rønning, Norsus AS
Helene Løvkvist Andersen
(no signature required)
Approved:
2 / 12
Product
Product description:
weber WX Waterproofing membrane is 1-component, ready-to-use waterproofing membrane for waterproofing wet rooms. It is suitable for wet rooms, such as
bathrooms and laundry rooms, and sauna floor waterproofing. Not suitable for swimming pools or areas around the pools, unheated spaces or for waterproofing sauna
walls or ceilings. Suitable substrates are stone-based surfaces, concrete and suitable boards. weberSmart work instructions 8-75 should be followed when waterproofing.
Hand applied. Available in 15 L package. GTIN 06415910039127.
Product specification
The composition of the product is described in the following table. Weight of packaging materials is given for 1 kg of product.
Materials
Dispersion 60-80%
Filler 10-30%
Additives 3-8%
Packaging, PP incl. 50% PCR 0,036kg
Packaging, metal (handle) 0,002kg
Packaging, PE 0,001kg
Packaging, cardboard 0,001kg
Packaging, pallet 0,050kg
Technical data:
weber WX Waterproofing membrane is part of weberSmart Waterproofing system which is VTT certified (VTT-C-12260-18).
Material consumption: 0,75 l/m² (membrane thickness 0,5 mm). The space details and substrate unevenness increases consumption significantly.
Density: Specific gravity: 1,25 kg/l
Minimum layer thickness: 0,5 mm.
More information: www.fi.weber/vedeneristyksen-ratkaisut-ja-tuotteet/nestemaiset-vedeneristeet-ja-epoksit/weber-wx-vedeneriste
Market:
Finland and Baltic countries
Reference service life, product
The reference service life of the product is similar to the service life of the building.
Reference service life, building
60 years
LCA: Calculation rules
Declared unit:
1 kg weber WX Waterproofing membrane (weber WX Vedeneriste)
Cut-off criteria:
All major raw materials and all the essential energy is included. The production processes for raw materials and energy flows with very small amounts (less than 1%) are
not included. These cut-off criteria do not​ apply for hazardous materials and substances.
Allocation:
The allocation is made in accordance with the provisions of EN 15804. Incoming energy and water and waste production in-house is allocated equally among all products
through mass allocation. Effects of primary production of recycled materials is allocated to the main product in which the material was used. The recycling process and
transportation of the material is allocated to this analysis.
Data quality:
Specific data for the product composition are provided by the manufacturer. The data represent the production of the declared product and were collected for EPD
development in the year of study. Background data is based on EPDs according to EN 15804 and different LCA databases. The data quality of the raw materials in A1 is
presented in the table below.
Materials Source Data quality Year
Additives ecoinvent 3.6 Database 2019
Packaging ecoinvent 3.6 Database 2019
Pigments ecoinvent 3.6 Database 2019
Water ecoinvent 3.6 Database 2019
Additives ecoinvent 3.6 Database 2020
3 / 12
System boundaries (X=included, MND=module not declared, MNR=module not relevant)
Construction Beyond the
Product stage installation Use stage End of life stage system
stage boundaries
A1 A2 A3 A4 A5 B1 B2 B3 B4 B5 B6 B7 C1 C2 C3 C4 D
X X X X X MND MND MND MND MND MND MND X X X X X
System boundary:
All processes from raw material extraction to product transport to the building site, assembly as well as end of life stage and phases beyond the system boundary (A1-A5,
C1-C4, D) are included in the analysis.
The production process comprises of mixing raw materials together. Ready mixed product is then packed into plastic pails with lid for delivery. Stage B is not considered.
At the end-of-life stage the impact of the product in building deconstruction is considered to be minor, therefore no impact is calculated in C1. Default waste scenario
from NPCR Part B Technical - Chemical products for building and construction industry is applied. Thus, at end-of-life, 10% of the product is collected for material
recycling and 90% is disposed into landfill.
System boundaries (cradle-to-gate with options) are illustrated in the picture below.
Additional technical information:
The LCA calculation has been made taking into account the fact that during the manufacturing process 100% renewable electricity is used. This 100% renewable
electricity bought is evidenced by Guarantee of Origin certificates (GOs) from LOS, valid for the study year (2021) and after.
Package contains 50% post-consumer recycled plastic, and can be recycled.
waR slairetam tropsnarT gnirutcafunaM tropsnarT ylbmessA e​sU ecnanetniaM riapeR tnemecalpeR tnemhsibrufeR lanoitarepO esu ygrene lanoitarepO esu retaw -eD noitcurtsnoc noitilomed tropsnarT etsaW gnissecorp lasopsiD -yrevoceR-esueR -gnilcyceR laitnetop
4 / 12
LCA: Scenarios and additional technical information
The following information describe the scenarios in the different modules of the EPD.
The results of stage A4 (transportation of product) in the table of this EPD refer to transportation in Finland (average distance 2021). This product may also be delivered to
the countries in the table "Additional A4 information". In order to adapt the impact of transportation to these countries, A4 figures from this EPD shall be multiplied by the
multiplication factors below.
At installation stage, no additional accessory was taken into account. Material loss is considered to be 0.
Due to minor impact in deconstruction phase, C1 is set 0. Transportation distance to waste disposal is assumed to be 30 km. It is assumed that 90% of the product is
disposed into landfill and 10% is collected and recycled.
Capacity utilisation Value
Transport from production place to user (A4) Distance (km) Fuel/Energy Consumption Unit
(incl. return) % (Liter/tonne)
Truck, over 32 tonnes, EURO 5 (km) 53,3 % 245 0,023 l/tkm 5,64
Ship, Freight, Transoceanic (km) 65,0 % 440 0,003 l/tkm 1,32
Additional A4 information Unit/Range Value
Multiplication factor
Tallinn, Estonia (truck 317 km / ferry 528 km) 1,28
GWP/A4
Multiplication factor
Riga, Latvia (truck 587 km / ferry 528 km) 2,21
GWP/A4
Multiplication factor
Kaunas, Lithuania (truck 847 km / ferry 528 km) 3,11
GWP/A4
Assembly (A5) Unit Value
Waste, cardboard and paper packaging, to
kg 0,00
average treatment (kg)
Waste, metal, to average treatment (kg) kg 0,00
Waste, plastic packaging, mixture, to average
kg 0,04
treatment (kg)
Waste, wood packaging, average treatment (kg) kg 0,05
Capacity utilisation Value
Transport to waste processing (C2) Distance (km) Fuel/Energy Consumption Unit
(incl. return) % (Liter/tonne)
Truck, over 32 tonnes, EURO 5 (km) 53,3 % 30 0,023 l/tkm 0,69
Waste processing (C3) Unit Value
Waste treatment of product after demolition (kg) kg/DU 0,10
Disposal (C4) Unit Value
Disposal of product in landfill (kg) kg/DU 0,90
Benefits and loads beyond the system
Unit Value
boundaries (D)
Substitution of primary aggregates with crushed
kg/DU 0,10
recycled inert products (kg)
5 / 12
LCA: Results
The LCA results are presented below for the declared unit defined on page 2 of the EPD document.
Environmental impact
Parameter Unit A1-A3 A4 A5 C1 C2 C3 C4 D
GWP-total kg CO2 -eq 2,27E+00 2,64E-02 4,33E-03 0 2,73E-03 7,20E-05 7,39E-03 -2,34E-04
GWP-fossil kg CO2 -eq 2,33E+00 2,64E-02 4,32E-03 0 2,73E-03 7,10E-05 7,38E-03 -2,29E-04
GWP-biogenic kg CO2 -eq -6,13E-02 1,03E-05 6,99E-06 0 1,12E-06 6,13E-07 8,62E-06 -4,57E-06
GWP-luluc kg CO2 -eq 1,39E-03 9,36E-06 5,84E-07 0 7,96E-07 9,83E-08 1,81E-06 -1,55E-07
ODP kg CFC11 -eq 1,20E-07 6,03E-09 4,00E-10 0 6,30E-10 1,40E-11 2,80E-09 -4,20E-11
AP mol H+ -eq 1,72E-02 2,28E-04 1,46E-05 0 1,15E-05 5,75E-07 6,57E-05 -2,06E-06
EP-FreshWater kg P -eq 2,54E-05 1,87E-07 2,25E-08 0 2,08E-08 4,49E-09 8,37E-08 -6,09E-09
EP-Marine kg N -eq 3,26E-03 6,12E-05 8,02E-06 0 3,45E-06 1,68E-07 2,44E-05 -7,15E-07
EP-Terrestial mol N eq 3,40E-02 6,80E-04 6,34E-05 0 3,81E-05 1,94E-06 2,69E-04 -8,40E-06
POCP kg NMVOC -eq 1,11E-02 1,96E-04 1,73E-05 0 1,23E-05 5,20E-07 7,71E-05 -2,22E-06
ADP-minerals&metals1 Kg Sb-eq 1,88E-05 4,11E-07 3,85E-08 0 4,66E-08 9,01E-10 6,65E-08 -2,03E-08
ADP-fossil1 MJ 6,07E+01 3,99E-01 2,85E-02 0 4,24E-02 2,21E-03 2,03E-01 -3,87E-03
WDP1 m3 2,83E+01 2,76E-01 6,77E-02 0 3,25E-02 2,43E-01 1,25E+00 -1,82E-01
GWP total Global Warming Potential total; GWP fossil Global Warming Potential fossil fuels ; GWP biogenic Global Warming Potential biogenic; GWP luluc Global W
Potential land use change; ODP Ozone Depletion; AP Acidification; EP freshwater Eutrophication aquatic freshwater; EP marine Eutrophication aquatic marine; EP
terrestrial Eutrophication terrestrial ;POCP Photochemical zone formation; ADPE Abiotic Depletion Potential minerals and metals; ADPf Abiotic Depletion Potential fossil
fuels; WDP Water Depletion Potential
"Reading example: 9,0 E-03 = 9,0*10-3 = 0,009"
*INA Indicator Not Assessed
1. The results of this environmental impact indicator shall be used with care as the uncertainties on these results are high or as there is limited experienced with the
indicator
Remarks to environmental impacts
Small amounts of unused product can be disposed along with household or construction waste after solidification following consultation with waste disposal facility
operator and the pertinent authorities, and adhering to the necessary technical regulations.
6 / 12
Additional environmental impact indicators
Parameter Unit A1-A3 A4 A5 C1 C2 C3 C4 D
PM Disease incidence 1,71E-07 1,96E-09 2,01E-10 0 2,40E-10 9,00E-12 1,40E-09 -4,40E-11
IRP2 kgBq U235 eq. 2,94E-02 1,74E-03 1,15E-04 0 1,85E-04 3,70E-05 9,27E-04 -3,55E-05
ETP-fw1 CTUe 3,26E+01 2,84E-01 3,01E-02 0 3,10E-02 1,56E-03 1,11E-01 -3,99E-03
HTP-c1 CTUh 2,03E-09 0,00E+00 2,00E-12 0 0,00E+00 0,00E+00 5,00E-12 0,00E+00
HTP-nc1 CTUh 6,43E-08 2,45E-10 1,07E-10 0 3,00E-11 1,00E-12 8,00E-11 -5,00E-12
SQP1 Pt 1,34E+01 4,04E-01 3,04E-02 0 4,86E-02 1,25E-03 7,82E-01 8,79E-03
PM Particulate Matter emissions; IRP Ionizing radiation – human health; ETP-fw Eco toxicity – freshwater; HTP-c Human toxicity – cancer effects; HTP-nc Human
toxicity – non cancer effects; SQP Soil Quality (dimensionless)
"Reading example: 9,0 E-03 = 9,0*10-3 = 0,009"
*INA Indicator Not Assessed
1. The results of this environmental impact indicator shall be used with care as the uncertainties on these results are high or as there is limited experienced with the
indicator
2. This impact category deals mainly with the eventual impact of low dose ionizing radiation on human health of the nuclear fuel cycle. It does not consider effects due
to possible nuclear accidents, occupational exposure nor due to radioactive waste disposal in underground facilities. Potential ionizing radiation from the soil, from
radon and from some construction materials is also not measured by this indicator.
7 / 12
Resource use
Parameter Unit A1-A3 A4 A5 C1 C2 C3 C4 D
PERE MJ 1,32E+00 4,72E-03 6,39E-04 0 5,34E-04 1,14E-03 7,27E-03 -9,07E-04
PERM MJ 7,10E-01 0,00E+00 0,00E+00 0 0,00E+00 0,00E+00 0,00E+00 0,00E+00
PERT MJ 2,03E+00 4,72E-03 6,39E-04 0 5,34E-04 1,14E-03 7,27E-03 -9,07E-04
PENRE MJ 6,41E+01 3,99E-01 2,85E-02 0 4,24E-02 2,21E-03 2,03E-01 -4,09E-03
PENRM MJ 1,40E+00 0,00E+00 0,00E+00 0 0,00E+00 0,00E+00 0,00E+00 0,00E+00
PENRT MJ 6,42E+01 3,99E-01 2,85E-02 0 4,24E-02 2,21E-03 2,03E-01 -4,09E-03
SM kg 3,15E-02 0,00E+00 1,41E-05 0 0,00E+00 1,90E-06 8,81E-05 -7,83E-06
RSF MJ 2,54E-02 1,61E-04 1,78E-05 0 1,87E-05 2,30E-05 1,51E-04 -1,85E-05
NRSF MJ 5,35E-03 6,32E-04 1,30E-04 0 6,26E-05 -1,42E-06 3,26E-04 -1,91E-05
FW m3 4,81E-02 4,22E-05 1,81E-05 0 4,83E-06 3,78E-06 2,50E-04 -1,42E-04
PERE Use of renewable primary energy excluding renewable primary energy resources used as raw materials; PERM Use of renewable primary energy resources used as
raw materials; PERT Total use of renewable primary energy resources; PENRE Use of non renewable primary energy excluding non-renewable primary energy resources
used as raw materials; PENRM Use of non renewable primary energy resources used as raw materials; PENRT Total use of non renewable primary energy resources; SM
Use of secondary materials; RSF Use of renewable secondary fuels; NRSF Use of non renewable secondary fuels; FW Use of net fresh water
"Reading example: 9,0 E-03 = 9,0*10-3 = 0,009"
*INA Indicator Not Assessed
8 / 12
End of life - Waste
Parameter Unit A1-A3 A4 A5 C1 C2 C3 C4 D
HWD kg 1,17E-02 2,12E-05 5,24E-04 0 2,32E-06 2,20E-07 1,43E-05 -9,34E-07
NHWD kg 3,50E-01 3,02E-02 1,92E-02 0 3,69E-03 6,96E-06 9,01E-01 -2,83E-05
RWD kg 3,39E-05 2,73E-06 1,71E-07 0 2,90E-07 2,33E-08 1,32E-06 -3,07E-08
HWD Hazardous waste disposed; NHWDNon-hazardous waste disposed; RWD Radioactive waste disposed;
"Reading example: 9,0 E-03 = 9,0*10-3 = 0,009"
*INA Indicator Not Assessed
End of life - Output flow
Parameter Unit A1-A3 A4 A5 C1 C2 C3 C4 D
CRU kg 0,00E+00 0,00E+00 0,00E+00 0 0,00E+00 0,00E+00 0,00E+00 0,00E+00
MFR kg 3,48E-03 0,00E+00 2,14E-02 0 0,00E+00 1,00E-01 8,03E-05 -1,83E-07
MER kg 3,10E-03 0,00E+00 1,92E-07 0 0,00E+00 2,30E-07 1,51E-06 -6,86E-06
EEE MJ 1,49E-02 0,00E+00 3,52E-02 0 0,00E+00 3,95E-07 1,25E-04 -1,66E-06
EET MJ 2,25E-01 0,00E+00 5,32E-01 0 0,00E+00 5,97E-06 1,89E-03 -2,50E-05
CRU Components for re-use; MFR Materials for recycling; MER Materials for energy recovery; EEE Exported electrical energy; EET Exported energy Thermal
"Reading example: 9,0 E-03 = 9,0*10-3 = 0,009"
*INA Indicator Not Assessed
Biogenic Carbon Content
Parameter Unit At the factory gate
Biogenic carbon content in product kg C 0,00E+00
Biogenic carbon content in accompanying packaging kg C 2,11E-02
Note: 1 kg biogenic carbon is equivalent to 44/12 kg CO2
9 / 12
Additional Norwegian requirements
Greenhouse gas emissions from the use of electricity in the manufacturing phase
National production mix from import, low voltage (production of transmission lines, in addition to direct emissions and losses in grid) of applied electricity for the
manufacturing process (A3).
Electricity mix Data source Amount Unit
Renewable electricity Saint-Gobain, based on 100% hydro power, with Guarantee of Origin from LOS 2021 (kWh) ecoinvent 3.6 4,26 g CO2-eq/kWh
Dangerous substances
The product contains no substances given by the REACH Candidate list or the Norwegian priority list.
Indoor environment
weber WX Waterproofing membrane is part of weberSmart Waterproofing system which has M1 indoor air emission classification granted by The Finnish Building
Information Foundation RTS (https://cer.rts.fi/en/m1-emission-class-for-building-material/).
Additional Environmental Information
Environmental impact indicators EN 15804+A1 and NPCR Part A v2.0
Parameter Unit A1-A3 A4 A5 C1 C2 C3 C4 D
GWP kg CO2 -eq 2,27E+00 2,61E-02 3,78E-03 0 2,70E-03 7,00E-05 7,23E-03 -2,45E-04
ODP kg CFC11 -eq 1,14E-07 5,05E-09 3,25E-10 0 5,10E-10 1,70E-11 2,25E-09 -3,80E-11
POCP kg C2H4-eq 5,76E-04 5,68E-06 6,61E-07 0 3,52E-07 1,56E-08 1,70E-06 -5,11E-08
AP kg SO2 -eq 1,39E-02 1,52E-04 8,48E-06 0 5,44E-06 2,63E-07 2,01E-05 -5,99E-07
EP kg PO43- -eq 1,20E-03 1,64E-05 3,20E-06 0 5,94E-07 3,48E-08 2,37E-06 -7,02E-08
ADPM kg Sb -eq 1,88E-05 4,11E-07 3,85E-08 0 4,66E-08 9,01E-10 6,65E-08 -2,03E-08
ADPE MJ 6,00E+01 3,92E-01 2,77E-02 0 4,16E-02 8,47E-04 1,95E-01 -3,87E-03
GWPIOBC kg CO2 -eq 2,15E+00 2,64E-02 0,00E+00 0 2,73E-03 0,00E+00 0,00E+00 -2,45E-04
GWP Global warming potential; ODP Depletion potential of the stratospheric ozone layer; POCP Formation potential of tropospheric photochemical oxidants; AP
Acidification potential of land and water; EP Eutrophication potential; ADPM Abiotic depletion potential for non fossil resources; ADPE Abiotic depletion​ potential for
fossil resources; GWP-IOBC/GHG Global warming potential calculated according to the principle of instantanious oxidation (except emissions and uptake of biogenic
carbon)
10 / 12
Bibliography
ISO 14025:2010 Environmental labels and declarations - Type III environmental declarations - Principles and procedures.
ISO 14044:2006 Environmental management - Life cycle assessment - Requirements and guidelines.
EN 15804:2012+A2:2019 Environmental product declaration - Core rules for the product category of construction products.
ISO 21930:2017 Sustainability in buildings and civil engineering works - Core rules for environmental product declarations of construction products.
ecoinvent v3, Allocation, cut-off by classification, Swiss Centre of Life Cycle Inventories.
Iversen et al., (2021) eEPD v2021.09 Background information for EPD generator tool system verification, LCA.no Report number: 07.21
Iversen et al., (2019) EPD generator for Saint-Gobain Weber and Scanspac - Background information and LCA data, LCA.no report number 05.18
Iversen et al., (2020) EPD generator for Saint-Gobain Weber Nordics and Scanspac Background information for customer application,
and LCA data – Supplementary report for modules A5, C and D, LCA.no report number 04.20
NPCR Part A: Construction products and services. Ver. 2.0, 24.03.2021 EPD Norway.
NPCR 009 Part B for technical-chemical products. Ver. 2.0 October 2021, EPD-Norge.
Program operator and publisher Phone: +47 23 08 80 00
The Norwegian EPD Foundation e-mail: post@epd-norge.no
Post Box 5250 Majorstuen, 0303 Oslo, Norway web: www.epd-norge.no
Owner of the declaration: Phone: +358400289933
anne.kaiser@saint-
Saint-Gobain Finland Oy e-mail:
gobain.com
P.O. Box 70, Fi-00381 Helsinki web: www.saint-gobain.fi
Author of the Life Cycle Assessment Phone: +47 916 50 916
LCA.no AS e-mail: post@lca.no
Dokka 6B, 1671 web: www.lca.no
Developer of EPD generator Phone: +47 916 50 916
LCA.no AS e-mail: post@lca.no
Dokka 6B,1671 Kråkerøy web: www.lca.no
ECO Platform Web: www.eco-platform.org
ECO Portal Web: ECO Portal
11 / 12
EPD for the best
environmental
decision
The Norwegian EPD Foundation
www.epd-norge.no
12 / 12
