ENVIRONMENTAL PRODUCT DECLARATION
as per ISO 14025 and EN 15804+A1
Owner of the Declaration ArcelorMittal Europe
Programme holder Institut Bauen und Umwelt e.V. (IBU)
Publisher Institut Bauen und Umwelt e.V. (IBU)
Declaration number EPD-ARC-20210245-CBA1-EN
Issue date 29.10.2021
Valid to 28.10.2026
XCarb® Recycled and renewably produced
Reinforcing steel in bars
ArcelorMittal Europe
www.ibu-epd.com | https://epd-online.com
Umwelt Produktdeklaration Name des Herstellers – Name des Produkts
General Information
ArcelorMittal Europe XCarb® Recycled and renewably
produced
Reinforcing steel in bars
Programme holder Owner of the declaration
IBU – Institut Bauen und Umwelt e.V. ArcelorMittal Europe-Long Products
Panoramastr. 1 66, rue de Luxembourg
10178 Berlin L-4221 Esch-sur-Alzette
Germany Luxembourg
Declaration number Declared product / declared unit
EPD-ARC-20210245-CBA1-EN 1 metric tonne of XCarb® Recycled and renewably
produced Reinforcing steel in bars.
This declaration is based on the product Scope:
category rules: The declaration applies to 1 metric tonne of
Structural steels, 30.11.2017 XCarb® Recycled and renewably produced Reinforcing
(PCR checked and approved by the SVR) steel in bars produced by ArcelorMittal.
Issue date The Life Cycle Assessment is based on data collected
29.10.2021 from one ArcelorMittal plant producing rebar (Warsaw
in Poland). It covers >95% of the annual production
with 2019 data for deliveries based on Guarantee of
Valid to
Origins renewable electricity supply.
28.10.2026
The owner of the declaration shall be liable for the
underlying information and evidence; the IBU shall not
be liable with respect to manufacturer information, life
cycle assessment data and evidences.
The EPD was created according to the specifications
of EN 15804+A1. In the following, the standard will be
simplified as EN 15804.
Verification
The standard EN 15804 serves as the core PCR
Independent verification of the declaration and data
according to ISO 14025:2010
Dipl. Ing. Hans Peters internally x externally
(chairman of Institut Bauen und Umwelt e.V.)
Dr. Alexander Röder Matthias Klingler
(Managing Director Institut Bauen und Umwelt e.V.)) (Independent verifier)
Product
Product description/Product definition (with the exception of Switzerland) the following legal
provisions apply:
This EPD applies to 1 metric tonne of XCarb™
Recycled and renewably produced Reinforcing steel in EN 10080:2005, Steel for the reinforcement of
bars for the building industry based on steel production concrete - Weldable reinforcing steel - General
in Electric Arc Furnace with renewable electricity
supply with Guarantee of Origins. The CE-marking takes into account the proof of
conformity with the respective harmonized standards
Rebar (Reinforcing Steel in bars, including standard based on the legal provisions above.
rebars, special rebars – Krybar®, rock bolt and tie bars For the application and use the respective national
- and threaded bars) covers carbon steel for provisions apply.
geotechnical use and the reinforcement of concrete.
The surface of rebars is patterned to form a better Application
bond with soil and concrete; in addition the ribs on
threaded bars, rock bolts and tie bars allow for bolting. Reinforcement bars are steel rods that are used as a
tension device in concrete. Typical applications are in
For the placing on the market in the European the construction of buildings, bridges, roads and other
Union/European Free Trade Association (EU/EFTA)
2 Environmental Product Declaration ArcelorMittal – XCarb® Recycled and renewably produced Reinforcing steel in bars
civil works (infrastructures, superstructures, etc.) as For the application and use the respective national
well as mining. provisions apply.
Technical Data For the application and use of the products the
following standards apply: EN 1992-1-1, EN 1992-1-2,
This EPD is valid for XCarb® Recycled and renewably EN 1992-2, EN 1992-3.
produced Reinforcing steel in bars of various steel
grades and different forms of delivery produced with a Base materials/Ancillary materials
certified supply of renewable electricity.
The base material of XCarb® Recycled and renewably
Performance data of the product in accordance with produced Reinforcing steel in bars is iron. Alloying
the Declaration of Performance. elements are added in the form of ferroalloys or metals
(most common elements are Manganese and Silicon).
Constructional data Some small quantities of other elements may be
present in the steel.
Name Value Unit No substances listed on the “Candidate List of
Density 7850 kg/m3 Substances of Very High Concern for Authorisation” by
Modulus of elasticity 210000 N/mm2 the European Chemicals Agency EC 1907-2006 are
Coefficient of thermal expansion 12 10-6K-1 contained in the steel in declarable quantities.
Thermal conductivity 48 W/(mK)
Melting point 1536 °C This product contains substances listed in the
Minimum yield strength 460 - 900 N/mm2 candidate list (date: 22.2.2021) exceeding 0.1
Tensile strength 483 - 1100 N/mm2 percentage by mass: no
Shear modulus 81000 N/mm²
Reference service life
A reference service life for XCarb® Recycled and
Product not harmonised in accordance with the CPR
renewably produced Reinforcing steel in bars is not
but in accordance with other provisions for
declared. These are construction products with many
harmonisation of the EU:
different applications purposes. The lifetime therefore
EN 10080:2005, Steel for the reinforcement of
will be limited by the service life of the work.
concrete - Weldable reinforcing steel - General (the
relevant test procedures are detailed in EN 10080).
LCA: Calculation rules
Declared Unit  Transport of resources and additives to the
 production site
The declaration refers to the declared unit of 1 metric
 Production processes on-site including
tonne of XCarb® Recycled and renewably produced
energy, production of additives, disposal of
Reinforcing steel in bars as specified in Part B
requirements on the EPD for reinforcing steel. production residues, and consideration of
related emissions
Foreground data for the production are integrated into  Recycling of production/manufacturing scrap.
the software model for the considered production Steel scrap is assumed to reach the end-of-
site/company. The LCI is assessed as per the annual
waste status once is shredded and sorted,
production data of ArcelorMittal Europe at the site
thus becomes input to the product system in
Warszawa.The background data are taken from GaBi
ts Documentation. the inventory.
Declared unit For the environmental impact, the use of green
electricity was calculated. The proportion of the
Name Value Unit electricity demand covered by green electricity in the
Declared unit 1 t total electricity demand of the on-site production at
Density 7850 kg/m3 Warszawa is 100%.
Conversion factor to 1 kg 0.001 -
Modules C3-C4 take into account the sorting and
shredding of after-use steel, as well as the
nonrecovered scrap due to sorting efficiency which is
System boundary landfilled. A conservative value of 10% landfill is
considered.
Type of the EPD: cradle-to-gate - with options.
Module A1-A3, Modules C3-C4 and Module D were Module D refers to the End-of-Life,
considered. including recycling.
Modules A1-A3 include the following: Comparability
 The provision of resources, additives, and Basically, a comparison or an evaluation of EPD data
energy is only possible if all the data sets to be compared
3 Environmental Product Declaration ArcelorMittal – XCarb® Recycled and renewably produced Reinforcing steel in bars
were created according to EN 15804 and the building For the life cycle modelling of the product under study,
context, respectively the product-specific the GaBi Software System for Life Cycle
characteristics of performance, are taken into account. Engineering, content version 2021.1, is used (GaBi
ts).
LCA: Scenarios and additional technical information
Current practice for the average rebar product consists
of 91% recycling, 1% reuse and 8% landfill according
to SteelConstruction-info.
This EPD considers a conservative approach of 90%
recycling and 10% landfill:
End of life (C3 - C4)
Name Value Unit
Landfilling 10 %
Reuse, recovery and/or recycling potentials (D),
relevant scenario information
Name Value Unit
Recycling 90 %
4 Environmental Product Declaration ArcelorMittal – XCarb® Recycled and renewably produced Reinforcing steel in bars
LCA: Results
DESCRIPTION OF THE SYSTEM BOUNDARY (X = INCLUDED IN LCA; MND = MODULE NOT DECLARED;
MNR = MODULE NOT RELEVANT)
BENEFITS AND
CONSTRUCTI LOADS
PRODUCT STAGE ON PROCESS USE STAGE END OF LIFE STAGE BEYOND THE
STAGE SYSTEM
BOUNDARIES
5 Environmental Product Declaration ArcelorMittal – XCarb® Recycled and renewably produced Reinforcing steel in bars
lairetam
waR
ylppus tropsnarT
gnirutcafunaM
eht
morf
tropsnarT
etis
eht
ot
etag
ylbmessA esU
ecnanetniaM
riapeR
tnemecalpeR tnemhsibrufeR
ygrene
lanoitarepO esu
retaw
lanoitarepO esu
noitcurtsnoc-eD
noitilomed tropsnarT
gnissecorp
etsaW
lasopsiD -esueR -yrevoceR -gnilcyceR laitnetop
A1 A2 A3 A4 A5 B1 B2 B3 B4 B5 B6 B7 C1 C2 C3 C4 D
X X X MND MND MND MND MNR MNR MNR MND MND MND MND X X X
RESULTS OF THE LCA - ENVIRONMENTAL IMPACT according to EN 15804+A1: 1 t XCarb™ Recycled
and renewably produced Reinforcing steel in bars
Parameter Unit A1-A3 C3 C4 D
Global warming potential [kg CO2-Eq.] 3.00E+2 1.60E+0 1.43E+0 2.46E+2
Depletion potential of the stratospheric ozone layer [kg CFC11-Eq.] 5.69E-11 4.69E-14 7.83E-15 5.75E-13
Acidification potential of land and water [kg SO2-Eq.] 8.66E-1 2.99E-3 8.57E-3 3.97E-1
Eutrophication potential [kg (PO4)3--Eq.] 6.24E-2 4.48E-4 9.72E-4 2.04E-2
Formation potential of tropospheric ozone photochemical
[kg ethene-Eq.] 5.79E-2 2.60E-4 6.58E-4 1.23E-1
oxidants
Abiotic depletion potential for non-fossil resources [kg Sb-Eq.] 1.89E-3 4.70E-7 1.44E-7 5.48E-4
Abiotic depletion potential for fossil resources [MJ] 3.25E+3 1.82E+1 1.95E+1 2.32E+3
RESULTS OF THE LCA - INDICATORS TO DESCRIBE RESOURCE USE according to EN 15804+A1: 1 t
XCarb™ Recycled and renewably produced Reinforcing steel in bars
Parameter Unit A1-A3 C3 C4 D
Renewable primary energy as energy carrier [MJ] 6.29E+3 1.22E+1 2.70E+0 -2.07E+2
Renewable primary energy resources as material utilization [MJ] 0.00E+0 0.00E+0 0.00E+0 0.00E+0
Total use of renewable primary energy resources [MJ] 6.29E+3 1.22E+1 2.70E+0 -2.07E+2
Non-renewable primary energy as energy carrier [MJ] 3.37E+3 2.82E+1 2.01E+1 2.25E+3
Non-renewable primary energy as material utilization [MJ] 0.00E+0 0.00E+0 0.00E+0 0.00E+0
Total use of non-renewable primary energy resources [MJ] 3.37E+3 2.82E+1 2.01E+1 2.25E+3
Use of secondary material [kg] 1.05E+3 0.00E+0 0.00E+0 0.00E+0
Use of renewable secondary fuels [MJ] 0.00E+0 0.00E+0 0.00E+0 0.00E+0
Use of non-renewable secondary fuels [MJ] 0.00E+0 0.00E+0 0.00E+0 0.00E+0
Use of net fresh water [m³] 4.57E-1 1.18E-2 4.95E-3 1.14E+0
RESULTS OF THE LCA – WASTE CATEGORIES AND OUTPUT FLOWS according to EN 15804+A1:
1 t XCarb™ Recycled and renewably produced Reinforcing steel in bars
Parameter Unit A1-A3 C3 C4 D
Hazardous waste disposed [kg] 1.57E-6 6.99E-9 2.13E-9 -6.28E-7
Non-hazardous waste disposed [kg] 5.86E+0 1.89E-2 1.00E+2 -2.71E+1
Radioactive waste disposed [kg] 3.30E-2 3.89E-3 2.10E-4 -8.16E-5
Components for re-use [kg] 0.00E+0 0.00E+0 0.00E+0 0.00E+0
Materials for recycling [kg] 0.00E+0 9.00E+2 0.00E+0 0.00E+0
Materials for energy recovery [kg] 0.00E+0 0.00E+0 0.00E+0 0.00E+0
Exported electrical energy [MJ] 0.00E+0 0.00E+0 0.00E+0 0.00E+0
Exported thermal energy [MJ] 0.00E+0 0.00E+0 0.00E+0 0.00E+0
References
EN 10080 EN 1992-1-2:2004, Eurocode 2: Design of concrete
EN 10080:2005, Steel for the reinforcement of structures - Part 1-2: General rules - Structural fire
concrete - Weldable reinforcing steel - General design
EN 1992-1-1 EN 1992-2
EN 1992-1-1:2004, Eurocode 2: Design of concrete EN 1992-2:2005, Eurocode 2 - Design of concrete
structures - Part 1-1: General rules and rules for structures - Concrete bridges - Design and detailing
buildings rules
EN 1992-1-2 EN 1992-3
EN 1992-3:2006, Eurocode 2 - Design of concrete
structures - Part 3: Liquid retaining and containment IBU 2021, General Instructions for the EPD
structures programme of Institut Bauen und Umwelt e.V. Version
2.0, Berlin: Institut Bauen und Umwelt e.V.,
Candidate List of Substances of Very High 2021www.ibu-epd.de
Concern for Authorisation
Regulation (EC) No 1907/2006 of the European IBU Part A
Parliament and of the Council on the Registration, PCR - Part A: Calculation rules for the Life Cycle
Evaluation, Authorisation and Restriction of Chemicals Assessment and Requirements on the Background
(REACH). https://echa.europa.eu/candidate-list-table Report, version 1.8, Institut Bauen und Umwelt e.V.,
www.bau-umwelt.com, 2019
EN 15804
EN 15804:2012-04+A1 2013, Sustainability of IBU Part B
construction works — Environmental Product PCR – Part B: Requirements of the EPD for Metal
Declarations — Core rules for the product category of Ceilings, Institut Bauen und Umwelt e.V., www.bau-
construction products. umwelt.com, 2019
ISO 14025 SteelConstruction-info
DIN EN ISO 14025:2011-10, Environmental labels and https://www.steelconstruction.info/The_recycling_and_
declarations — Type III environmental declarations — reuse_survey
Principles and procedures.
Worldsteel 2011
GaBi ts Life cycle assessment (LCA) methodology report
GaBi ts dataset documentation for the GaBi Software http://www.worldsteel.org/publications/
System and Database for Life Cycle Engineering,
thinkstep AG, Leinfelden-Echterdingen, 2021
(http://documentation.gabi-software.com/)
IBU 2021
6 Environmental Product Declaration ArcelorMittal – XCarb® Recycled and renewably produced Reinforcing steel in bars
Publisher
Institut Bauen und Umwelt e.V. Tel +49 (0)30 3087748- 0
Panoramastr. 1 Fax +49 (0)30 3087748- 29
10178 Berlin Mail info@ibu-epd.com
Germany Web www.ibu-epd.com
Programme holder
Institut Bauen und Umwelt e.V. Tel +49 (0)30 - 3087748- 0
Panoramastr 1 Fax +49 (0)30 – 3087748 - 29
10178 Berlin Mail info@ibu-epd.com
Germany Web www.ibu-epd.com
Author of the Life Cycle
Assessment Tel +49 711 341817-0
Sphera Solutions GmbH Fax +49 711 341817-25
Hauptstraße 111- 113 Mail info@sphera.com
70771 Leinfelden-Echterdingen Web www.sphera.com
Germany
Owner of the Declaration
ArcelorMittal Europe – Long Tel +352 5313 2142
Products – Bars & Rods Fax -
Rue de Luxemburg 66 Mail
4221 Esch-sur-Alzette longeurope.barsandrods@arcelo
Luxembourg rmittal.com
Web barsandrods.arcelormittal.com
