ENVIRONMENTAL PRODUCT DECLARATION
as per ISO 14025 and EN 15804+A2
Owner of the Declaration ArcelorMittal Europe – Flat Products
Programme holder Institut Bauen und Umwelt e.V. (IBU)
Publisher Institut Bauen und Umwelt e.V. (IBU)
Declaration number EPD-ARC-20220236-CBA1-EN
Issue date 16.11.2022
Valid to 15.11.2027
XCarb® Recycled and Renewably produced hot dip
galvanized steel with Magnelis® Coating
ArcelorMittal
www.ibu-epd.com | https://epd-online.com
Umwelt Produktdeklaration Name des Herstellers – Name des Produkts
General Information
ArcelorMittal XCarb® Recycled and Renewably
Produced Hot dip galvanized steel with
Magnelis® Coating
Programme holder Owner of the declaration
IBU – Institut Bauen und Umwelt e.V. ArcelorMittal Europe – Flat Products
Hegelplatz 1 24-26 Boulevard d’Avranches
10117 Berlin L-1160 Luxembourg
Germany Luxembourg
Declaration number Declared product / declared unit
EPD-ARC-20220236-CBA1-EN The declared unit is 1 metric ton of XCarb® Recycled
and Renewably Produced Magnelis® coated steel (1.5
mm steel thickness with 310 g/m² Magnelis® coating)
This declaration is based on the product Scope:
category rules: This declaration applies to 1 metric tonne of
Structural steels, 11.2017 XCarb® Recycled and Renewably Produced
(PCR checked and approved by the SVR) Magnelis® coated steel produced at ArcelorMittal.
Issue date The Life Cycle Assessment is based on the LCA model
16.11.2022 and data for ArcelorMittal XCarb® Recycled and
Renewably Produced Hot Rolled Coils, coupled with
downstream processes at ArcelorMittal plants,
Valid to
covering 100% of the production of the declared
15.11.2027
product.
The owner of the declaration shall be liable for the
underlying information and evidence; the IBU shall not
be liable with respect to manufacturer information, life
cycle assessment data and evidences.
The EPD was created according to the specifications
of EN 15804+A2. In the following, the standard will be
simplified as EN 15804.
Verification
The standard EN 15804 serves as the core PCR
Independent verification of the declaration and data
according to ISO 14025:2011
Dipl. Ing. Hans Peters internally x externally
(chairman of Institut Bauen und Umwelt e.V.)
Dr. Alexander Röder Matthias Klingler
(Managing Director Institut Bauen und Umwelt e.V.)) (Independent verifier)
Product
Product description/Product definition XCarb® Recycled and Renewably Produced hot dip
This Environmental Product Declaration refers to galvanized steel with Magnelis® Coating is compliant
XCarb® Recycled and Renewably Produced hot dip with EN 10346.
galvanized steel with Magnelis® Coating. The product
is a double-sided hot-dip galvanized carbon steel The coated steel is available in a very wide range of
coated on both sides with a zinc-aluminium- steel grades (steels for cold forming and deep drawing
magnesium alloy. This alloy, composed of 93.5 % zinc, applications, structural steels and High Strength Low
3.5 % aluminium and 3 % magnesium, is applied by Alloy steels), and coating masses (from 70 to 800
means of a continuous hot dip galvanizing process. A g/m²). ZM is the symbol used in EN 10346 to refer to
post-treatment (passivation, thin organic coating and/or Zinc Aluminium Magnesium coatings to which
oiling) can also be applied on the product. Magnelis® coated steel belongs.
This chemical composition has been selected to
provide an excellent corrosion resistance.
2 Environmental Product Declaration ArcelorMittal – XCarb® Recycled and Renewably Produced hot dip galvanized steel
with Magnelis® coating
steel grade used as substrate and measured according
For the use and application of the product, the to EN ISO 6892. The corrosion resistance performance
respective national provisions at the place of use can be evaluated with different indoor and outdoor
apply. tests. One of the most common tests is the ‘Salt Spray
Test’ defined according to EN ISO 9227/ASTM B-117.
Application Constructional data
XCarb® Recycled and Renewably Produced hot dip The following table refers to steel properties without
galvanized steel with Magnelis® coating can be used the coating. Properties with coating differ according to
in various industrial applications, such as: thickness. If necessary, specific characteristics can be
 Construction: structural or non-structural obtained at
profiles, roofing & cladding, decking, cable http://industry.arcelormittal.com/catalogue/E35/EN.
trays, expanded metal, gratings, composite
Name Value Unit
flooring, concrete moulds
Density 7850 kg/m3
 Road and railway infrastructure: safety Modulus of elasticity 210000 N/mm2
barriers, protection equipment, sound Coefficient of thermal expansion 12 10-6K-1
 insulation wall panels, walls providing Thermal conductivity 48 W/(mK)
protection against hail Melting point 1536 °C
 Agriculture and farming: barns, greenhouse
structures, agricultural equipment
Performance data of the product with respect to its
 Solar energy generation: structures for
characteristics in accordance with the relevant
photovoltaic plants technical provision (no CE-marking).
 Tubular applications: structural tubes for
scaffolding, road signals, poles. Base materials/Ancillary materials
The base material of XCarb® Recycled and
Renewably Produced hot dip galvanized with
The coated steel is delivered in wide coils, slit coils,
Magnelis® coating is iron. Alloying elements are added
blanks or sheets. It can be processed by all
on the form of ferroalloys or metals. The metallic
conventional processing operations used for hot dip
coating includes only zinc, aluminium and magnesium.
galvanized steel: bending, drawing, clinching, profiling,
stamping, welding etc.
This product comes from a production process flow
which only uses XCarb® Recycled and Renewably
The friction coefficient of XCarb® Recycled and
Produced Hot Rolled Coil. This pre-material will only
Renewably Produced hot dip galvanized steel with
be transported by sea or train to the ArcelorMittal
Magnelis® coating is lower than the one of standard
finishing mills outside Spain.
hot dip galvanized steel and is stable during cold
forming operations.
The substrates can be made of different steel grades
(DX51D to DX57D, S220GD to S550GD, HX260LAD
Technical Data
to HX500LAD, EN 10346) with steel thicknesses
Due to its 3 % magnesium content, XCarb® Recycled
ranging between 0.36 mm and 6.0 mm.
and Renewably Produced hot dig galvanized with
Magnelis® coating offers self-healing on cut edges and
Detailed steel and coating properties and chemical
corrosion resistance in chloride and ammonia
compositions are available at:
atmospheres. This high corrosion resistance means
http://industry.arcelormittal.com/catalogue/E35/EN.
that less metallic coating is required to ensure an
equivalent corrosion protection than with standard hot
This product contains substances listed in the
dip galvanized steels.
candidate list (date 02.06.2022) above 0.1 mass
percent: No.
The coating process can apply various thickness of the
Zinc Aluminium Magnesium layer, up to 800 g/m² (total
Reference service life
of both sides).
Hot dip galvanized coated steels are used in
construction with many different application purposes.
Specific mechanical properties are defined for each
The service life therefore will be limited by the
3 Environmental Product Declaration ArcelorMittal – XCarb® Recycled and Renewably Produced hot dip galvanized steel
with Magnelis® coating
application and corresponding service. At the end of
life, they will be recovered and recycled into a new
steel product.
LCA: Calculation rules
Declared Unit  Recycling of production/manufacturing scrap.
The declaration refers to the functional unit of 1 metric Steel scrap is assumed to reach the end-of-
ton of double-sided XCarb® Recycled and Renewably
waste status once is shredded and sorted,
Produced hot dip galvanized steel with Magnelis®
thus becoming input to the product system in
coating, packed and ready to be transported from
the inventory.
ArcelorMittal to its clients as specified in Part B
requirements on the EPD.
Module C1 assumes a generic multi-story building
The results are calculated based on a 1.5mm steel demolition scenario. Module C2 includes impacts of
thickness with 310 g/m² Magnelis® coating. The steel assumed distances of 100 km from the demolition site
substrate has been elaborated from an XCarb® of a scrap processing plant and 200 km from this plant
Recycled and Renewably Produced Hot Rolled Coil. to the disposal. In both cases, empty returns of
transport were assumed.
Declared unit
Name Value Unit Module C3 takes into account the sorting and
Declared unit 1 t shredding of after-use steel to allow its orientation
Thickness 1.5 mm towards the recycling solutions. This process will also
Density 7828 kg/m3 produce losses due to efficiency that will be oriented
towards landfill sites. A conservative value of 2 %
The product described refers to the average annual landfill is then considered in C4.
production at ArcelorMittal in Europe for the reference
year of 2021. The results are within a 10 % variation. Module C4 takes into account the waste disposal
including physical pre-treatment and management of
the disposal site. Steel is an inert material which does
System boundary not require any specific treatment on disposal site.
Type of EPD: cradle to gate with modules C1–C4 and
module D (A1-A3, C and D) Module D refers to the end of life of the structural
steel, including reuse and recycling
Modules A1-A3 of the XCarb® Recycled and
Renewably Produced hot dip galvanized steel with Comparability
Magnelis® coating production include: Basically, a comparison or an evaluation of EPD data
 The provision of resources, additives, and is only possible if all the data sets to be compared
energy were created according to EN 15804 and the building
context, respectively the product-specific
 Transport of resources and additives to the
characteristics of performance, are taken into account.
production site
 Transport of intermediate products within
ArcelorMittal sites For life cycle modelling of the considered
 Production processes on site include energy, products, GaBi ts software version 10.6.1.35 was used
production of additives, disposal of production with GaBi database 2022.2. This database contains
consistent and documented datasets available in Gabi
residues, and consideration of related
Documentation
emissions.
LCA: Scenarios and additional technical information
Characteristic product properties
Information on biogenic carbon Information on describing the biogenic Carbon
The declared product does not contain any biogenic Content at factory gate
carbon. Name Value Unit
Biogenic Carbon Content in
0 kg C
Product packaging is adapted to the way the product product
will be transported, its intended use, its thickness and Biogenic Carbon Content in
1.46 kg C
width, and the customer's request. accompanying packaging
For modelling, a conservative scenario was employed,
considering the following amounts of packaging
materials.
 Steel – 0.796 kg
 Plastic – 0.075 kg
End of life (C1 - C4)
 Timber – 1.5 kg
Current practice for the average hot dip galvanized
 Cardboard – 1.73 kg.
steel consists of 98 % recycling and 2 % landfill
4 Environmental Product Declaration ArcelorMittal – XCarb® Recycled and Renewably Produced hot dip galvanized steel
with Magnelis® coating
according to the European Commission Technical
Steel Research.
Name Value Unit
Recycling 980 kg
Landfilling 20 kg
Reuse, recovery and/or recycling potentials (D),
relevant scenario information
Name Value Unit
Recycling 98 %
5 Environmental Product Declaration ArcelorMittal – XCarb® Recycled and Renewably Produced hot dip galvanized steel
with Magnelis® coating
LCA: Results
DESCRIPTION OF THE SYSTEM BOUNDARY (X = INCLUDED IN LCA; ND = MODULE OR INDICATOR NOT
DECLARED; MNR = MODULE NOT RELEVANT)
BENEFITS AND
CONSTRUCTI LOADS
PRODUCT STAGE ON PROCESS USE STAGE END OF LIFE STAGE BEYOND THE
STAGE SYSTEM
BOUNDARIES
6 Environmental Product Declaration ArcelorMittal – XCarb® Recycled and Renewably Produced hot dip galvanized steel
with Magnelis® coating
lairetam
waR
ylppus tropsnarT
gnirutcafunaM
eht
morf
tropsnarT
etis
eht
ot
etag
ylbmessA esU
ecnanetniaM
riapeR
tnemecalpeR tnemhsibrufeR
ygrene
lanoitarepO esu
retaw
lanoitarepO esu
noitcurtsnoc-eD
noitilomed tropsnarT
gnissecorp
etsaW
lasopsiD -esueR -yrevoceR -gnilcyceR laitnetop
A1 A2 A3 A4 A5 B1 B2 B3 B4 B5 B6 B7 C1 C2 C3 C4 D
X X X ND ND ND ND MNR MNR MNR ND ND X X X X X
RESULTS OF THE LCA - ENVIRONMENTAL IMPACT according to EN 15804+A2: 1 ton XCarb® Recycled
and Renewably Produced hot dip galvanized steel with Magnelis® coating
Core Indicator Unit A1-A3 C1 C2 C3 C4 D
Global warming potential - total [kg CO2-Eq.] 7.97E+2 4.35E+1 2.13E+1 1.53E+0 2.90E-1 -5.42E+1
Global warming potential - fossil fuels [kg CO2-Eq.] 7.94E+2 4.32E+1 2.11E+1 1.52E+0 2.98E-1 -5.43E+1
Global warming potential - biogenic [kg CO2-Eq.] 2.43E+0 1.83E-3 1.53E-2 5.40E-3 -8.84E-3 8.68E-2
GWP from land use and land use change [kg CO2-Eq.] 1.60E-1 2.82E-1 1.45E-1 9.36E-4 5.51E-4 -1.45E-2
Depletion potential of the stratospheric ozone layer [kg CFC11-Eq.] 8.93E-8 1.33E-11 2.12E-12 1.99E-11 7.01E-13 1.50E-10
Acidification potential, accumulated exceedance [mol H+-Eq.] 2.51E+0 2.46E-1 1.27E-1 3.75E-3 2.12E-3 -1.49E-1
Eutrophication, fraction of nutrients reaching freshwater
[kg P-Eq.] 2.17E-3 1.52E-4 7.70E-5 4.31E-6 5.06E-7 -9.69E-6
end compartment
Eutrophication, fraction of nutrients reaching marine end
[kg N-Eq.] 5.64E-1 1.19E-1 6.20E-2 1.03E-3 5.41E-4 -3.10E-2
compartment
Eutrophication, accumulated exceedance [mol N-Eq.] 6.08E+0 1.32E+0 6.87E-1 1.10E-2 5.94E-3 -3.36E-1
Formation potential of tropospheric ozone photochemical
[kg NMVOC-Eq.] 1.66E+0 2.31E-1 1.20E-1 2.82E-3 1.64E-3 -1.04E-1
oxidants
Abiotic depletion potential for non-fossil resources [kg Sb-Eq.] 9.13E-2 4.45E-6 2.17E-6 3.84E-7 3.06E-8 1.19E-6
Abiotic depletion potential for fossil resources [MJ] 9.26E+3 5.82E+2 2.83E+2 2.68E+1 3.91E+0 -4.03E+2
Water (user) deprivation potential, deprivation-weighted [m³ world-Eq
1.75E+2 6.26E-1 2.41E-1 3.11E-1 3.27E-2 1.14E+0
water consumption (WDP) deprived]
RESULTS OF THE LCA - INDICATORS TO DESCRIBE RESOURCE USE according to EN 15804+A2: 1 ton
XCarb® Recycled and Renewably Produced hot dip galvanized steel with Magnelis® coating
Indicator Unit A1-A3 C1 C2 C3 C4 D
Renewable primary energy as energy carrier [MJ] 2.06E+4 4.44E+1 1.96E+1 1.38E+1 5.86E-1 5.87E+1
Renewable primary energy resources as material utilization [MJ] 0.00E+0 0.00E+0 0.00E+0 0.00E+0 0.00E+0 0.00E+0
Total use of renewable primary energy resources [MJ] 2.06E+4 4.44E+1 1.96E+1 1.38E+1 5.86E-1 5.87E+1
Non-renewable primary energy as energy carrier [MJ] 9.27E+3 5.85E+2 2.84E+2 2.68E+1 3.91E+0 -4.08E+2
Non-renewable primary energy as material utilization [MJ] 0.00E+0 0.00E+0 0.00E+0 0.00E+0 0.00E+0 0.00E+0
Total use of non-renewable primary energy resources [MJ] 9.27E+3 5.85E+2 2.84E+2 2.68E+1 3.91E+0 -4.08E+2
Use of secondary material [kg] 9.52E+2 0.00E+0 0.00E+0 0.00E+0 0.00E+0 2.76E+1
Use of renewable secondary fuels [MJ] 0.00E+0 0.00E+0 0.00E+0 0.00E+0 0.00E+0 0.00E+0
Use of non-renewable secondary fuels [MJ] 0.00E+0 0.00E+0 0.00E+0 0.00E+0 0.00E+0 0.00E+0
Use of net fresh water [m³] 4.26E+0 5.04E-2 2.27E-2 1.32E-2 9.93E-4 -3.52E-2
RESULTS OF THE LCA – WASTE CATEGORIES AND OUTPUT FLOWS according to EN 15804+A2:
1 ton XCarb® Recycled and Renewably Produced hot dip galvanized steel with Magnelis® coating
Indicator Unit A1-A3 C1 C2 C3 C4 D
Hazardous waste disposed [kg] 3.00E-6 4.07E-9 1.50E-9 7.90E-8 0.00E+0 2.02E-8
Non-hazardous waste disposed [kg] 2.06E+1 1.03E-1 4.63E-2 1.90E-2 2.00E+1 -7.70E-1
Radioactive waste disposed [kg] 2.87E-1 2.86E-3 5.27E-4 3.95E-3 4.35E-5 6.74E-3
Components for re-use [kg] 0.00E+0 0.00E+0 0.00E+0 0.00E+0 0.00E+0 0.00E+0
Materials for recycling [kg] 0.00E+0 0.00E+0 0.00E+0 9.80E+2 0.00E+0 0.00E+0
Materials for energy recovery [kg] 0.00E+0 0.00E+0 0.00E+0 0.00E+0 0.00E+0 0.00E+0
Exported electrical energy [MJ] 0.00E+0 0.00E+0 0.00E+0 0.00E+0 0.00E+0 0.00E+0
Exported thermal energy [MJ] 0.00E+0 0.00E+0 0.00E+0 0.00E+0 0.00E+0 0.00E+0
RESULTS OF THE LCA – additional impact categories according to EN 15804+A2-optional:
1 ton XCarb® Recycled and Renewably Produced hot dip galvanized steel with Magnelis® coating
Indicator Unit A1-A3 C1 C2 C3 C4 D
Potential incidence of disease due to PM emissions [Disease
ND ND ND ND ND ND
Incidence]
Potential Human exposure efficiency relative to U235 [kBq U235-
ND ND ND ND ND ND
Eq.]
Potential comparative toxic unit for ecosystems [CTUe] ND ND ND ND ND ND
Potential comparative toxic unit for humans - cancerogenic [CTUh] ND ND ND ND ND ND
Potential comparative toxic unit for humans - not cancerogenic [CTUh] ND ND ND ND ND ND
Potential soil quality index [-] ND ND ND ND ND ND
Note: 952 kg of scrap are used in the manufacturing of 1 metric ton of XCarb® RRP hot dip galvanized steel with
Magnelis® coating. After use, 980 kg steel are recycled, and 20 kg are landfilled. The potential environmental
impact calculated for module D depends on the net amount of scrap left in the system, which is 980-952 = 28 kg.
This means that the system has a net output of 28 kg of scrap, which is shown in module D as an environmental
credit or burden depending on the impact category.
The additional and optional impact categories in accordance with EN 15804-A2 have not been declared, as this
is not required in accordance with PCR Part A.
Disclaimer 1 – for the indicator “Potential Human exposure efficiency relative to U235”.
This impact category deals mainly with the eventual impact of low-dose ionizing radiation on human health of the
nuclear fuel cycle. It does not consider effects due to possible nuclear accidents, occupational exposure or
radioactive waste disposal in underground facilities. Potential ionizing radiation from the soil, from radon and from
some construction materials is also not measured by this indicator.
Disclaimer 2 – for the indicators “abiotic depletion potential for nonfossil resources”, “abiotic depletion potential for
fossil resources”, “water (user) deprivation potential, deprivation-weighted water consumption”,
“potential comparative toxic unit for ecosystems”, “potential comparative toxic unit for humans – cancerogenic”,
“Potential comparative toxic unit for humans not cancerogenic”, “potential soil quality index”.
The results of this environmental impact indicator shall be used with care as the uncertainties on these results are
high as there is limited experienced with the indicator.
References
ASTM B-117 steel research, 2001-12.
ASTM B-117:2019 - Standard Practice for Operating
Salt Spray (Fog) Apparatus GaBi ts Documentation
GaBi ts dataset documentation for the GaBi datasets
EN 1993-1-3 for Life Cycle Engineering. LBP, University of Stuttgart
EN 1993-1-3:2006 - Eurocode 3 - Design of steel and PE International, 2011.
structures - Part 1-3: General rules - Supplementary http://documentation.gabi-software.com/.
rules for cold-formed members and sheeting.
GaBi ts Software
EN 10346 GaBi ts Software and Databases for Life Cycle
EN10346:2015 - Continuously hot-dip coated steel flat Engineering. LBP, University of Stuttgart and PE
products for cold forming - Technical delivery International, 2013.
conditions
IBU 2021
EN 15804 Institut Bauen und Umwelt e.V.: General Instructions
EN 15804:2012+A2:2019+AC:2021, Sustainability of for the EPD programme of Institut Bauen und Umwelt
construction works — Environmental Product e.V., Version 2.0, Berlin: Institut Bauen und Umwelt
Declarations — Core rules for the product category of e.V., 2021.
construction products. www.ibu-epd.com
EN ISO 6892 PCR Part A
ISO 6892:2019 - Metallic materials — Tensile testing PCR - Part A: Calculation Rules for the Life Cycle
Assessment and Requirements on the Project Report,
EN ISO 9227 Institut Bauen und Umwelt e.V., 2021.
EN ISO 9227:2017 - Corrosion tests in artificial www.bauumwelt.com
atmospheres – Salt spray tests
PCR Part B
ISO 14025 PCR - Part B: Requirements of the EPD for Structural
EN ISO 14025:2011, Environmental labels and steels, Institut Bauen und Umwelt e.V., 2017.
declarations — Type III environmental declarations — www.bauumwelt.com
Principles and procedures.
Worldsteel 2011
Candidate list - REACH Life cycle assessment (LCA) methodology report for
Regulation (EC) No 1907/2006 of the European steel products.
Parliament and of the Council on the Registration, © World Steel Association 2017.
Evaluation, Authorisation and Restriction https://worldsteel.org/wp-content/uploads/Life-cycle-
of Chemicals (REACH). inventory-methodology-report.pdf
https://echa.europa.eu/candidate-list-table
European Commission Technical Steel Research
Sansom, M.and Meijer, J.:Life-cycle assessment (LCA)
for steel construction, European Commission technical
7 Environmental Product Declaration ArcelorMittal – XCarb® Recycled and Renewably Produced hot dip galvanized steel
with Magnelis® coating
Publisher
Institut Bauen und Umwelt e.V. Tel +49 (0)30 3087748- 0
Hegelplatz 1 Fax +49 (0)30 3087748- 29
10117 Berlin Mail info@ibu-epd.com
Germany Web www.ibu-epd.com
Programme holder
Institut Bauen und Umwelt e.V. Tel +49 (0)30 - 3087748- 0
Hegelplatz 1 Fax +49 (0)30 – 3087748 - 29
10117 Berlin Mail info@ibu-epd.com
Germany Web www.ibu-epd.com
Author of the Life Cycle
Assessment Tel +352 4792-1
ArcelorMittal Europe – Flat Fax -
Products Mail
Boulevard d’Avranches 24-26 flateurope.technical.assistance@
1160 Luxembourg arcelormittal.com
Luxembourg Web flateurope.arcelormittal.com/
Owner of the Declaration
ArcelorMittal Europe – Flat Tel +352 4792-1
Products Fax -
Boulevard d’Avranches 24-26 Mail
1160 Luxembourg flateurope.technical.assistance@
Luxembourg arcelormittal.com
Web flateurope.arcelormittal.com/
