ENVIRONMENTAL PRODUCT DECLARATION
as per ISO 14025 and EN 15804+A2
Owner of the Declaration ArcelorMittal Europe – Flat Products
Programme holder Institut Bauen und Umwelt e.V. (IBU)
Publisher Institut Bauen und Umwelt e.V. (IBU)
Declaration number EPD-ARC-20220319-CBA1-EN
Issue date 15.12.2022
Valid to 14.12.2027
XCarb® recycled and renewably produced organic coated
steel coils Granite® and Estetic®
ArcelorMittal
www.ibu-epd.com | https://epd-online.com
Umwelt Produktdeklaration Name des Herstellers – Name des Produkts
General Information
ArcelorMittal XCarb® recycled and renewably
produced organic coated steel coils
Programme holder Owner of the declaration
IBU – Institut Bauen und Umwelt e.V. ArcelorMittal Europe – Flat Products
Hegelplatz 1 24-26 Boulevard d’Avranches
10117 Berlin L-1160 Luxembourg
Germany Luxembourg
Declaration number Declared product / declared unit
EPD-ARC-20220319-CBA1-EN The declared unit is 1 metric ton of XCarb® recycled
and renewably produced organic coated steel from the
Granite® and Estetic® range.
This declaration is based on the product Scope:
category rules: This declaration applies to 1 metric ton of XCarb®
Structural steels, 11.2017 recycled and renewably produced organic coated steel
(PCR checked and approved by the SVR) coil (Granite® and Estetic®).
Issue date The Life Cycle Assessment is based on the LCA model
15.12.2022 and data for ArcelorMittal XCarb® recycled and
renewably produced hot rolled coils, coupled with
downstream processes at ArcelorMittal plants,
Valid to
representing 95 % of the production XCarb® recycled
14.12.2027
and renewably produced organic coated steel
(Granite® and Estetic®).
The owner of the declaration shall be liable for the
underlying information and evidence; the IBU shall not
be liable with respect to manufacturer information, life
cycle assessment data and evidences.
The EPD was created according to the specifications
of EN 15804+A2. In the following, the standard will be
simplified as EN 15804.
Verification
The standard EN 15804 serves as the core PCR
Independent verification of the declaration and data
according to ISO 14025:2011
Dipl. Ing. Hans Peters internally x externally
(chairman of Institut Bauen und Umwelt e.V.)
Dr. Alexander Röder Matthias Klingler
(Managing Director Institut Bauen und Umwelt e.V.)) (Independent verifier)
Product
Product description/Product definition cladding) and indoor use (home appliances, general
This Environmental Product Declaration refers to industry and building components) processed by
XCarb® recycled and renewably produced organic drawing, roll forming, bending, flanging, or spinning.
coated steel coils from the Granite® and Estetic®
range. The Granite® and Estetic® range combines Granite® & Estetic® prepainted steels are made of a
metallic coated steel substrates with a protective Zinc or Optigal® (respectively Z & ZM according to EN
organic coating system to create robust colour-coated 10346 standard) metallic coated steel with coating
products with high weathering resistance and therefore weights ranging from 60 to 350 g/m², combined with an
longer lifetime. additional organic coating with thicknesses as follows:
 Top side 25 μm to 75 μm for Granite® and 15
Granite® & Estetic® prepainted steels are delivered in μm to 55 μm for Estetic®
compliance with standard EN 10169.
 Back side 5 μm to 75 μm for Granite® and
5μm to 25 μm for Estetic®
These two families of prepainted products are
available in a wide range of steel grades aimed for
architectural buildings for outdoor use (roofing,
2 Environmental Product Declaration ArcelorMittal – XCarb® recycled and renewably produced organic coated steel coils
Granite® and Estetic®
More info available at:
https://industry.arcelormittal.com/catalogue#family_f
thickness. If necessary, specific characteristics can be
For the use and application of the product, the obtained at
respective national provisions at the place of use https://industry.arcelormittal.com/catalogue/F10/EN.
apply, in Germany for example the building codes of
the federal states and the corresponding national Name Value Unit
specifications. Density 7850 kg/m3
Modulus of elasticity 210000 N/mm2
Application Coefficient of thermal expansion 12 10-6K-1
Organic-coated steel is used in all sectors of industry. Thermal conductivity 48 W/(mK)
In building and construction, it is used as profiles Melting point 1536 °C
for cladding, roofing, tiles, gutters etc.
ArcelorMittal’s coloured organic coated steel Performance data of the product with respect to its
coils comprise hot dip galvanized coils as a substrate characteristics are in accordance with the relevant
over which organic coatings are applied. The coils are technical provision (no CE-marking).
then delivered to manufacturers for shaping into
end products to be included in building works, Base materials/Ancillary materials
generally to precise dimensions, thereby avoiding
losses on the construction site. The base material of organic-coated steel coils is iron.
Alloying elements are added in the form of ferroalloys
Technical Data or metals. The metallic coating includes either zinc (Z)
The thickness of coatings (i.e. metallic layer and or an alloy made of zinc, aluminium, and magnesium
organic coating) varies according to the intended end (ZM) as defined in EN 10346 standard. The organic
use of the products. Granite® is suitable for outdoor coatings are made from polyester, polyurethane or
applications whereas Estetic® is preferred for indoor polyvinylidene fluoride (PVDF) resins.
applications. Granite® and Estetic® products can be
processed by bending, profiling, cold roll forming and XCarb® recycled and renewably produced organic
deep drawing without damaging the top surface. They coated steel coils (Granite® and Estetic®) originate
can be joined using techniques such as clinching, from a production process flow which only
riveting and adhesive bonding. These products are in uses XCarb® recycled and renewably produced hot
compliance with EN 10169 standard. rolled coil as pre-material. This pre-material will only be
transported by sea or train to the ArcelorMittal finishing
Detailed steel and coating properties and chemical mills outside Spain.
compositions for the different products in the Granite®
and Estetic® range are available at: ArcelorMittal’s organic coated steel is produced in full
 https://industry.arcelormittal.com/catalogue/F compliance with the European REACH Regulation
30/EN, (Registration, Evaluation, Authorization and Restriction
 https://industry.arcelormittal.com/catalogue/F of Chemicals). In particular, all coatings and surface
treatments used for Granite® and Estetic® are free of
40/EN and
hexavalent chromium compounds, which are
 https://industry.arcelormittal.com/catalogue/F
substances of very high concern (SVHC) included in
20/EN.
REACH Annexe XIV, and hazardous heavy metals
(Pb, Hg and Cd).
Constructional data This product contains substances listed in
The following table refers to steel properties without the candidate list (date 02.06.2022) above 0.1 mass
the coating. Properties with coating differ according to percent: No.
3 Environmental Product Declaration ArcelorMittal – XCarb® recycled and renewably produced organic coated steel coils
Granite® and Estetic®
construction with many different application purposes.
Reference service life The lifetime therefore will be limited by the application
A reference service life for XCarb® recycled and and corresponding service. At the end of life, they will
renewably produced organic coated steel from the be recovered and recycled into a new steel product.
Granite® and Estetic® range is not declared.
Hot dip galvanized organic coated steels are used in
LCA: Calculation rules
Declared Unit production residues, and consideration of
The declaration refers to the functional unit of 1 metric related emissions.
ton of double-sided XCarb® recycled and renewably
 Recycling of production/manufacturing scrap.
produced organic coated steel from the Granite® and
Steel scrap is assumed to reach the end-of-
Estetic® range, packed and ready to be transported
waste status once is shredded and sorted,
from ArcelorMittal to its clients as specified in Part B
requirements of the EPD. thus becoming input to the product system in
the inventory.
The results are calculated based on a 0.47 mm steel
thickness with 225 g/m² metallic coating and 40 μm
Module C1 assumes a generic multi-story building
organic coating thickness (total on both sides). Prior to
demolition scenario.
the coating steps, the steel substrate has been cold
rolled from an XCarb® recycled and renewably
Module C2 includes impacts of assumed distances of
produced hot rolled coil.
100 km from the demolition site of a scrap processing
plant and 200 km from this plant to the disposal. In
Declared unit
both cases, empty returns of transport were assumed.
Name Value Unit
Declared unit 1 t
Module C3 takes into account the sorting and
Thickness (of steel) 0.47 mm
shredding of after-use steel to allow its orientation
For conversion to square meters, 1 metric ton of the
towards the recycling solutions. This process will also
declared unit is equivalent to 251.5 m2.
produce losses due to efficiency that will be oriented
towards landfill sites. A conservative value of 2 %
The product described refers to the average annual
landfill is then considered in C4.
production at ArcelorMittal in Europe for the reference
year of 2021. For Global Warming Potential (Total) the
Module C4 takes into account the waste disposal
results are within a 10 % variation.
including physical pre-treatment and management of
the disposal site. Steel is an inert material which does
not require any specific treatment on the disposal site.
System boundary
Type of EPD: cradle to gate with modules C1–C4 and
Module D refers to the end of life of structural steel,
module D (A1-A3, C and D)
including reuse and recycling.
Modules A1-A3 of the steel and coating production
Comparability
include:
Basically, a comparison or an evaluation of EPD data
 The provision of resources, additives, and
is only possible if all the data sets to be compared
energy were created according to EN 15804 and the building
 Transport of resources and additives to the context, respectively the product-specific
production site characteristics of performance, are taken into account.
 Transport of intermediate products within
ArcelorMittal sites
For life cycle modelling of the considered
 Production processes on site including products, GaBi ts software version 10.6.1.35 was used
energy, production of additives, disposal of with GaBi database 2022.1. This database contains
consistent and documented datasets available in Gabi
Documentation
LCA: Scenarios and additional technical information
Characteristic product properties considering the following amounts of packaging
Information on biogenic carbon materials.
The declared product does not contain any biogenic  Steel – 0.796 kg
carbon.  Plastic – 0.075 kg
 Timber – 1.5 kg
Product packaging is adapted to the way the product
 Cardboard – 1.73 kg.
will be transported, its intended use, its thickness and
width, and the customer's request.
For modelling, a conservative scenario was employed, Information on describing the biogenic Carbon
Content at factory gate
4 Environmental Product Declaration ArcelorMittal – XCarb® recycled and renewably produced organic coated steel coils
Granite® and Estetic®
Name Value Unit
Biogenic Carbon Content in
0 kg C
product
Biogenic Carbon Content in
1.46 kg C
accompanying packaging
Current practice for the average hot dip galvanized
steel consist of 98 % recycling and 2 % landfill
according to the European Commission Technical
Steel Research.
End of life (C1 - C4)
Current practice for the average organic coated steel
consists of 98 % recycling and 2 % landfill according to
the European Commission Technical Steel Research.
Name Value Unit
Recycling 980 kg
Landfilling 20 kg
Reuse, recovery and/or recycling potentials (D),
relevant scenario information
Name Value Unit
Recycling 98 %
5 Environmental Product Declaration ArcelorMittal – XCarb® recycled and renewably produced organic coated steel coils
Granite® and Estetic®
LCA: Results
DESCRIPTION OF THE SYSTEM BOUNDARY (X = INCLUDED IN LCA; ND = MODULE OR INDICATOR NOT
DECLARED; MNR = MODULE NOT RELEVANT)
BENEFITS AND
CONSTRUCTI LOADS
PRODUCT STAGE ON PROCESS USE STAGE END OF LIFE STAGE BEYOND THE
STAGE SYSTEM
BOUNDARIES
6 Environmental Product Declaration ArcelorMittal – XCarb® recycled and renewably produced organic coated steel coils
Granite® and Estetic®
lairetam
waR
ylppus tropsnarT
gnirutcafunaM
eht
morf
tropsnarT
etis
eht
ot
etag
ylbmessA esU
ecnanetniaM
riapeR
tnemecalpeR tnemhsibrufeR
ygrene
lanoitarepO esu
retaw
lanoitarepO esu
noitcurtsnoc-eD
noitilomed tropsnarT
gnissecorp
etsaW
lasopsiD -esueR -yrevoceR -gnilcyceR laitnetop
A1 A2 A3 A4 A5 B1 B2 B3 B4 B5 B6 B7 C1 C2 C3 C4 D
X X X ND ND ND ND MNR MNR MNR ND ND X X X X X
RESULTS OF THE LCA - ENVIRONMENTAL IMPACT according to EN 15804+A2: 1 ton XCarb® recycled
and renewably produced organic coated steel (Granite® and Estetic®)
Core Indicator Unit A1-A3 C1 C2 C3 C4 D
Global warming potential - total [kg CO2-Eq.] 1.03E+3 4.35E+1 2.13E+1 1.53E+0 2.90E-1 -1.40E+2
Global warming potential - fossil fuels [kg CO2-Eq.] 1.03E+3 4.32E+1 2.11E+1 1.52E+0 2.98E-1 -1.40E+2
Global warming potential - biogenic [kg CO2-Eq.] 0.00E+0 1.83E-3 1.53E-2 5.40E-3 -8.84E-3 2.24E-1
GWP from land use and land use change [kg CO2-Eq.] 2.93E-1 2.82E-1 1.45E-1 9.36E-4 5.51E-4 -3.75E-2
Depletion potential of the stratospheric ozone layer [kg CFC11-Eq.] 8.59E-8 1.33E-11 2.12E-12 1.99E-11 7.01E-13 3.88E-10
Acidification potential, accumulated exceedance [mol H+-Eq.] 3.07E+0 2.46E-1 1.27E-1 3.75E-3 2.12E-3 -3.84E-1
Eutrophication, fraction of nutrients reaching freshwater
[kg P-Eq.] 2.96E-3 1.52E-4 7.70E-5 4.31E-6 5.06E-7 -2.50E-5
end compartment
Eutrophication, fraction of nutrients reaching marine end
[kg N-Eq.] 7.06E-1 1.19E-1 6.20E-2 1.03E-3 5.41E-4 -8.01E-2
compartment
Eutrophication, accumulated exceedance [mol N-Eq.] 7.56E+0 1.32E+0 6.87E-1 1.10E-2 5.94E-3 -8.67E-1
Formation potential of tropospheric ozone photochemical
[kg NMVOC-Eq.] 2.29E+0 2.31E-1 1.20E-1 2.82E-3 1.64E-3 -2.67E-1
oxidants
Abiotic depletion potential for non-fossil resources [kg Sb-Eq.] 2.16E-1 4.45E-6 2.17E-6 3.84E-7 3.06E-8 3.08E-6
Abiotic depletion potential for fossil resources [MJ] 1.39E+4 5.82E+2 2.83E+2 2.68E+1 3.91E+0 -1.04E+3
Water (user) deprivation potential, deprivation-weighted [m³ world-Eq
2.20E+2 6.26E-1 2.41E-1 3.11E-1 3.27E-2 2.93E+0
water consumption (WDP) deprived]
RESULTS OF THE LCA - INDICATORS TO DESCRIBE RESOURCE USE according to EN 15804+A2: 1 ton
XCarb® recycled and renewably produced organic coated steel (Granite® and Estetic®)
Indicator Unit A1-A3 C1 C2 C3 C4 D
Renewable primary energy as energy carrier [MJ] 2.06E+4 4.44E+1 1.96E+1 1.38E+1 5.86E-1 1.52E+2
Renewable primary energy resources as material utilization [MJ] 6.00E+1 0.00E+0 0.00E+0 0.00E+0 0.00E+0 -2.00E-1
Total use of renewable primary energy resources [MJ] 2.07E+4 4.44E+1 1.96E+1 1.38E+1 5.86E-1 1.51E+2
Non-renewable primary energy as energy carrier [MJ] 1.39E+4 5.85E+2 2.84E+2 2.68E+1 3.91E+0 -1.05E+3
Non-renewable primary energy as material utilization [MJ] 4.00E+1 0.00E+0 0.00E+0 0.00E+0 0.00E+0 1.00E+0
Total use of non-renewable primary energy resources [MJ] 1.40E+4 5.85E+2 2.84E+2 2.68E+1 3.91E+0 -1.05E+3
Use of secondary material [kg] 9.09E+2 0.00E+0 0.00E+0 0.00E+0 0.00E+0 7.11E+1
Use of renewable secondary fuels [MJ] 0.00E+0 0.00E+0 0.00E+0 0.00E+0 0.00E+0 0.00E+0
Use of non-renewable secondary fuels [MJ] 0.00E+0 0.00E+0 0.00E+0 0.00E+0 0.00E+0 0.00E+0
Use of net fresh water [m³] 5.44E+0 5.04E-2 2.27E-2 1.32E-2 9.93E-4 -9.10E-2
RESULTS OF THE LCA – WASTE CATEGORIES AND OUTPUT FLOWS according to EN 15804+A2:
1 ton XCarb® recycled and renewably produced organic coated steel (Granite® and Estetic®)
Indicator Unit A1-A3 C1 C2 C3 C4 D
Hazardous waste disposed [kg] 3.75E-6 4.07E-9 1.50E-9 7.90E-8 0.00E+0 5.21E-8
Non-hazardous waste disposed [kg] 2.25E+1 1.03E-1 4.63E-2 1.90E-2 2.00E+1 -1.99E+0
Radioactive waste disposed [kg] 5.48E-1 2.86E-3 5.27E-4 3.95E-3 4.35E-5 1.74E-2
Components for re-use [kg] 0.00E+0 0.00E+0 0.00E+0 0.00E+0 0.00E+0 0.00E+0
Materials for recycling [kg] 0.00E+0 0.00E+0 0.00E+0 9.80E+2 0.00E+0 0.00E+0
Materials for energy recovery [kg] 0.00E+0 0.00E+0 0.00E+0 0.00E+0 0.00E+0 0.00E+0
Exported electrical energy [MJ] 0.00E+0 0.00E+0 0.00E+0 0.00E+0 0.00E+0 0.00E+0
Exported thermal energy [MJ] 0.00E+0 0.00E+0 0.00E+0 0.00E+0 0.00E+0 0.00E+0
RESULTS OF THE LCA – additional impact categories according to EN 15804+A2-optional:
1 ton XCarb® recycled and renewably produced organic coated steel (Granite® and Estetic®)
Indicator Unit A1-A3 C1 C2 C3 C4 D
Potential incidence of disease due to PM emissions [Disease
ND ND ND ND ND ND
Incidence]
Potential Human exposure efficiency relative to U235 [kBq U235-
ND ND ND ND ND ND
Eq.]
Potential comparative toxic unit for ecosystems [CTUe] ND ND ND ND ND ND
Potential comparative toxic unit for humans - cancerogenic [CTUh] ND ND ND ND ND ND
Potential comparative toxic unit for humans - not cancerogenic [CTUh] ND ND ND ND ND ND
Potential soil quality index [-] ND ND ND ND ND ND
Note: 909 kg of scrap are used in the manufacturing of 1 metric ton of XCarb® recycled and renewably produced
organic coated steel (Granite® and Estetic®). After use, 980 kg of steel are recycled, and 20 kg are landfilled. The
potential environmental impact calculated for module D depends on the net amount of scrap left in the system,
which is 980-909 = 71 kg. This means that the system has a net output of 71 kg of scrap, which is shown in
module D as an environmental credit or burden depending on the impact category.
The additional and optional impact categories in accordance with EN 15804-A2 have not been declared, as this
is not required in accordance with PCR Part A.
Disclaimer 1 – for the indicator “Potential Human exposure efficiency relative to U235”.
This impact category deals mainly with the eventual impact of low-dose ionizing radiation on human health of the
nuclear fuel cycle. It does not consider effects due to possible nuclear accidents, occupational exposure or
radioactive waste disposal in underground facilities. Potential ionizing radiation from the soil, [GRL1] radon and
from some construction materials is also not measured by this indicator.
Disclaimer 2 – for the indicators “abiotic depletion potential for nonfossil resources”, “abiotic depletion potential for
fossil resources”, “water (user) deprivation potential, deprivation-weighted water consumption”,
“potential comparative toxic unit for ecosystems”, “potential comparative toxic unit for humans – cancerogenic”,
“Potential comparative toxic unit for humans not cancerogenic”, “potential soil quality index”.
The results of this environmental impact indicator shall be used with care as the uncertainties on these results are
high as there is limited experience with the indicator.
References
EN10169 IBU 2021
EN10169:2022 - Continuously organic coated (coil Institut Bauen und Umwelt e.V.: General Instructions
coated) steel flat products - Technical delivery for the EPD programme of Institut Bauen und Umwelt
conditions e.V., Version 2.0, Berlin: Institut Bauen und Umwelt
e.V., 2021.
EN10346 www.ibu-epd.com
EN10346:2015 - Continuously hot-dip coated steel flat
products for cold forming - Technical delivery PCR Part A
conditions PCR - Part A: Calculation Rules for the Life Cycle
Assessment and Requirements on the Project Report,
EN 15804 Institut Bauen und Umwelt e.V., 2021.
EN 15804:2012+A2:2019+AC:2021, Sustainability of www.bauumwelt.com
construction works — Environmental Product
Declarations — Core rules for the product category of PCR Part B
construction products. PCR - Part B: Requirements of the EPD for Structural
steels, Institut Bauen und Umwelt e.V., 2017.
ISO 14025 www.bauumwelt.com
EN ISO 14025:2011, Environmental labels and
declarations — Type III environmental declarations — Candidate list - REACH
Principles and procedures. Regulation (EC) No 1907/2006 of the European
Parliament and of the Council on the Registration,
European Commission Technical Steel Research Evaluation, Authorisation and Restriction
Sansom, M.and Meijer, J.:Life-cycle assessment (LCA) of Chemicals (REACH).
for steel construction, European Commission technical https://echa.europa.eu/candidate-list-table
steel research, 2001-12.
Worldsteel 2011
GaBi ts Documentation Life cycle assessment (LCA) methodology report for
GaBi ts dataset documentation for the GaBi datasets steel products.
for Life Cycle Engineering. LBP, University of Stuttgart © World Steel Association 2017.
and PE International, 2011. https://worldsteel.org/wp-content/uploads/Life-cycle-
http://documentation.gabi-software.com/. inventory-methodology-report.pdf
GaBi ts Software
GaBi ts Software and Databases for Life Cycle
Engineering. LBP, University of Stuttgart and PE
International, 2013.
7 Environmental Product Declaration ArcelorMittal – XCarb® recycled and renewably produced organic coated steel coils
Granite® and Estetic®
Publisher
Institut Bauen und Umwelt e.V. Tel +49 (0)30 3087748- 0
Hegelplatz 1 Fax +49 (0)30 3087748- 29
10117 Berlin Mail info@ibu-epd.com
Germany Web www.ibu-epd.com
Programme holder
Institut Bauen und Umwelt e.V. Tel +49 (0)30 - 3087748- 0
Hegelplatz 1 Fax +49 (0)30 – 3087748 - 29
10117 Berlin Mail info@ibu-epd.com
Germany Web www.ibu-epd.com
Author of the Life Cycle
Assessment Tel +352 4792-1
ArcelorMittal Europe – Flat Fax -
Products Mail
Boulevard d’Avranches 24-26 flateurope.technical.assistance@
1160 Luxembourg arcelormittal.com
Luxembourg Web flateurope.arcelormittal.com/
Owner of the Declaration
ArcelorMittal Europe – Flat Tel +352 4792-1
Products Fax -
Boulevard d’Avranches 24-26 Mail
1160 Luxembourg flateurope.technical.assistance@
Luxembourg arcelormittal.com
Web flateurope.arcelormittal.com/
