Environmental product declaration
in accordance with ISO 14025 and EN 15804+A2
XCC-X2-NU, X2-015-VR
Owner of the declaration: Program operator:
TROX Group The Norwegian EPD Foundation
Product: Declaration number:
XCC-X2-NU, X2-015-VR
Registration number:
Declared unit:
1 pcs Issue date:
This declaration is based on Product Category Rules: Valid to:
CEN Standard EN 15804:2012+A2:2019 serves as core
EPD Software:
PCR
The Norwegian EPD Foundation LCA.no EPD generator ID: 152223
NPCR 030:2021 Part B for ventilation components
1 / 13
General information
Product Owner of the declaration:
XCC-X2-NU, X2-015-VR TROX Group
Contact person: Alina Buchner
Phone: +49 2845 2020
e-mail: productsustainability-de@troxgroup.com
Program operator: Manufacturer:
Post Box 5250 Majorstuen, 0303 Oslo, Norway TROX Group
The Norwegian EPD Foundation Heinrich-Trox-Platz 1
Phone: +47 23 08 80 00 47506 Neukirchen-Vluyn, Germany
web: post@epd-norge.no
Declaration number: Place of production:
TROX GmbH - Werk Anholt
Gendringer Str. 85
46419 Isselburg, Germany
This declaration is based on Product Category Rules: Management system:
CEN Standard EN 15804:2012+A2:2019 serves as core PCR ISO 9001, ISO 14001:2015, ISO 50001:2018
NPCR 030:2021 Part B for ventilation components
Statement of liability: Organisation no:
The owner of the declaration shall be liable for the underlying DE 120250070
information and evidence. EPD Norway shall not be liable with respect
to manufacturer information, life cycle assessment data and
evidences.​
Declared unit: Issue date:
1 pcs XCC-X2-NU, X2-015-VR
Declared unit with option: Valid to:
A1-A3,A4,C1,C2,C3,C4,D
Year of study:
2022
Functional unit: Comparability:
EPD of construction products may not be comparable if they not
comply with EN 15804 and seen in a building context.
General information on verification of EPD from EPD tools: Development and verification of EPD:
Independent verification of data, other environmental information The declaration is created using EPD tool lca.tools ver EPD2022.03,
and the declaration according to ISO 14025:2010, § 8.1.3 and § 8.1.4. developed by LCA.no. The EPD tool is integrated in the company's
Verification of each EPD is made according to EPD-Norway’s management system and has been approved by EPD Norway.
guidelines for verification and approval requiring that tools are i)
integrated into the company's environmental management system, ii) Developer of EPD: Klaus Niklas
the procedures for use of the EPD tool are approved by EPD-Norway,
Reviewer of company-specific input data and EPD:​ Alina Buchner
and iii) the process is reviewed annually by an independent third
party verifier. See Appendix G of EPD-Norway's General Programme
Instructions for further information on EPD tools
Verification of EPD tool: Approved:
Independent third party verification of the EPD tool, background data
and test-EPD in accordance with EPDNorway's procedures and
guidelines for verification and approval of EPD tools.
Third party verifier:
Alexander Borg, Asplan Viak AS
(no signature required)
2 / 13
Product
Product description:
TROX X-CUBE X2 Compact Unit Air handling unit (AHU) with a plug&play compact design for conditioning and process air. Energy label
certification according to the AHU Directive 01 and Eurovent.
AHUs can be customized to meet the needs of different applications. Due to the small size and the variable versions with vertical or horizontal
duct connection, installation is possible in the smallest of spaces. The slim units fit largely through standard doors and are easy to transport. With
the help of the rotary heat exchanger, the product achieves particular efficiency.
The units are supplied ready for connection and can be configured and commissioned via X-CUBE control.
Product specification
XCC-X2-NU, X2-015-VR
Vertical compact unit with heat recovery wheel, integrated heater, ODA/ETH filter, EC-fans, outside ODA/EHH damper.
Factory mounted control components complete with wiring and tubing. Housing with double-walled sandwich panels made of galv. sheet metal,
dimensionally stabilised and inlay-reinforced, as well as being powder-coated as described.
This EPD deals with a special configuration of an AHU. It includes the environmental data of the product series XCC-X2NU.
Due to the possibility of customised configuration, other variants may have different material compositions and a different total weight. The
following represents a representative dataset of the most sold variant in the declared sales year (X2-015-VR).
Materials kg %
Adhesive and sealant 5,30 1,47
Electronic - Cable 0,88 0,24
Electronic - Sensor 0,96 0,27
Electronic - Switch 0,24 0,07
Electronic - Unspecified 27,00 7,52
Extruded Polystyrene (XPS) 0,43 0,12
Filter, mineral based 0,87 0,24
Insulation, Mineral based 10,09 2,81
Metal - Aluminium 26,92 7,49
Metal - Brass 0,71 0,20
Metal - Copper 3,20 0,89
Metal - Galvanized Steel 254,87 70,94
Metal - Stainless steel 7,05 1,96
Metal - Steel 0,86 0,24
Motor 1,18 0,33
Plastic - Acrylonitrile butadiene styrene (ABS) 2,50 0,70
Plastic - Nylon (PA) 0,19 0,05
Plastic - Polyamide 0,10 0,03
Plastic - Polycarbonate (PC) 0,18 0,05
Plastic - Polyoxymethylene (POM) 0,01 0,00
Plastic - Polypropylene (PP) 0,07 0,02
Plastic - Polystyrene (PS) 0,73 0,20
Plastic - Polyurethane (PUR) 0,82 0,23
Plastic - Polyvinyl chloride (PVC) 0,21 0,06
Powder coating 11,83 3,29
Product label - supercalendered 0,01 0,00
Rubber, natural (Latex) 0,02 0,01
Rubber, synthetic 2,01 0,56
Textile - Cotton 0,02 0,01
Total 359,26
Packaging kg %
Packaging - Pallet 30,00 90,91
Packaging - Plastic 3,00 9,09
Total incl. packaging 392,26
Technical data:
Nominal size (B,H,L) 776x1543x1638
Nominal volume flow 1700 m³/h
Duct connection 450x300
Nominal data fan 230 V, 50 Hz, 0,5 kW, 1,8 A
Fan typ: EC
Market:
Europe
3 / 13
Reference service life, product
20-25 years.
Reference service life, building or construction works
60 years.
LCA: Calculation rules
Declared unit:
1 pcs XCC-X2-NU, X2-015-VR
Cut-off criteria:
All major raw materials and all the essential energy is included. The production processes for raw materials and energy flows with very small
amounts (less than 1%) are not included. These cut-off criteria do not​ apply for hazardous materials and substances.
Allocation:
The allocation is made in accordance with the provisions of EN 15804. Energy, water and waste production in-house is allocated equally among all
products through mass allocation. Effects of primary production of recycled materials is allocated to the main product in which the material was
used. The recycling process and transportation of the material is allocated to this analysis.
Data quality:
Specific data for the product composition are provided by the manufacturer. The data represent the production of the declared product and were
collected for EPD development in the year of study. Background data is based on EPDs according to EN 15804 and different LCA databases. The
data quality of the raw materials in A1 is presented in the table below.
Materials Source Data quality Year
Adhesive and sealant ecoinvent 3.6 Database 2019
Electronic - Cable ecoinvent 3.6 Database 2019
Electronic - Switch ecoinvent 3.6 Database 2019
Electronic - Unspecified ecoinvent 3.6 Database 2019
Extruded Polystyrene (XPS) ecoinvent 3.6 Database 2019
Filter, mineral based ecoinvent 3.6 Database 2019
Insulation, Mineral based ecoinvent 3.6 Database 2019
Metal - Aluminium ecoinvent 3.6 Database 2019
Metal - Brass ecoinvent 3.6 Database 2019
Metal - Copper ecoinvent 3.6 Database 2019
Metal - Stainless steel ecoinvent 3.6 Database 2019
Metal - Steel ecoinvent 3.6 Database 2019
Packaging - Pallet ecoinvent 3.6 Database 2019
Packaging - Plastic ecoinvent 3.6 Database 2019
Plastic - Acrylonitrile butadiene styrene (ABS) ecoinvent 3.6 Database 2019
Plastic - Nylon (PA) ecoinvent 3.6 Database 2019
Plastic - Polyamide ecoinvent 3.6 Database 2019
Plastic - Polycarbonate (PC) ecoinvent 3.6 Database 2019
Plastic - Polyoxymethylene (POM) ecoinvent 3.6 Database 2019
Plastic - Polypropylene (PP) ecoinvent 3.6 Database 2019
Plastic - Polystyrene (PS) ecoinvent 3.6 Database 2019
Plastic - Polyurethane (PUR) ecoinvent 3.6 Database 2019
Plastic - Polyvinyl chloride (PVC) ecoinvent 3.6 Database 2019
Powder coating ecoinvent 3.6 Database 2019
Product label - supercalendered ecoinvent 3.6 Database 2019
Rubber, natural (Latex) ecoinvent 3.6 Database 2019
Rubber, synthetic ecoinvent 3.6 Database 2019
Textile - Cotton ecoinvent 3.6 Database 2019
Metal - Galvanized Steel ecoinvent 3.6 Database 2020
Motor Modified ecoinvent 3.6 Database 2019
Supplier data +
Electronic - Sensor Product composition + ecoinvent 3.6 2019
database
4 / 13
System boundaries (X=included, MND=module not declared, MNR=module not relevant)
Construction Beyond the system
Product stage Use stage End of life stage
installation stage boundaries
A1 A2 A3 A4 A5 B1 B2 B3 B4 B5 B6 B7 C1 C2 C3 C4 D
X X X X MND MND MND MND MND MND MND MND X X X X X
System boundary:
Additional technical information:
The devices in the X-CUBE X2 series are the ideal solution for volume flows of 600 to 25,000 m³/h (0.17 to 6.9 m³/s). They are freely configurable
and can be used for all air treatment processes. The compact, pre-configured X-CUBE X2 compact models in 12 sizes also impress with their
technical features.
The X-CUBE X2 can be equipped with a rotary heat exchanger, a plate heat exchanger or a KV system.
Excellent design - available in white or anthracite.
Vibration-damped base frame (optional) eliminates the need for costly insulation on site.
High stability and appliance base strength.
Low weight facilitates transport and installation.
Excellent hygiene properties thanks to smooth interior surfaces and small gaps.
Robust and flexible locking system for doors and inspection panels.
The X-CUBE X2 is equipped with the new control software X-CUBE control 2.0 control software. The device can be operated via a high-
performance touch panel and connected to the TROX systems X-AIRCONTROL, TROXNETCOM and X-TAIRMINAL.
The monitoring functions of X-CUBE control 2.0 with their automatic status messages enable convenient system control around the clock. Via
BACnet IP or Modbus TCP/IP, the X-CUBE X2 is seamlessly integrated into the building management system. Thanks to this universal networking
capability, the performance of the air handling unit can be controlled as required. Optimum comfort is combined with maximum energy savings.
waR slairetam tropsnarT gnirutcafunaM tropsnarT ylbmessA e​sU ecnanetniaM riapeR tnemecalpeR tnemhsibrufeR lanoitarepO ygrene esu lanoitarepO esu retaw -eD noitcurtsnoc noitilomed tropsnarT etsaW gnissecorp lasopsiD -yrevoceR-esueR laitnetop-gnilcyceR
5 / 13
LCA: Scenarios and additional technical information
The following information describe the scenarios in the different modules of the EPD.
Capacity utilisation Value
Transport from production place to user (A4) Distance (km) Fuel/Energy Consumption Unit
(incl. return) % (Liter/tonne)
Truck, 16-32 tonnes, EURO 6 (km) 36,7 % 800 0,043 l/tkm 34,40
De-construction demolition (C1) Unit Value
Demolition of building per kg of ventilation
kg/DU 359,26
product (kg)
Capacity utilisation Value
Transport to waste processing (C2) Distance (km) Fuel/Energy Consumption Unit
(incl. return) % (Liter/tonne)
Truck, 16-32 tonnes, EURO 6 (km) 36,7 % 50 0,043 l/tkm 2,15
Waste processing (C3) Unit Value
Materials to recycling (kg) kg 266,57
Waste treatment per kg Bulk iron waste, excluding
kg 1,18
reinforcement, sorting plant (kg)
Waste treatment per kg Electronic scrap,
kg 28,21
incineration (kg)
Waste treatment per kg Hazardous waste,
kg 8,57
incineration (kg)
Waste treatment per kg Non-hazardous waste,
kg 0,02
incineration (kg)
Waste treatment per kg of waste cable, manual
kg 0,88
treatment (kg)
Waste treatment per kg plastic, industrial
electronics, municipal incineration with fly ash kg 1,25
extraction (kg)
Waste treatment per kg Plastics, incineration (kg) kg 1,23
Waste treatment per kg Polyethylene (PE),
kg 0,23
incineration (kg)
Waste treatment per kg Polyethylene
terephthalate (PET), incineration with fly ash kg 0,15
extraction (kg)
Waste treatment per kg Polyoxymethylene (POM),
kg 0,00
incineration with fly ash extraction (kg)
Waste treatment per kg Polypropylene (PP),
kg 0,03
incineration (kg)
Waste treatment per kg Polyvinylchloride (PVC),
kg 0,11
incineration with fly ash extraction (kg)
Waste treatment per kg Rubber, municipal
kg 1,12
incineration with fly ash extraction (kg)
6 / 13
Disposal (C4) Unit Value
Landfilling of ashes from incineration of
Electronic scrap, process of ashes and residues kg 19,79
(kg)
Landfilling of ashes from incineration of Non-
hazardous waste, process per kg ashes and kg 0,01
residues (kg)
Landfilling of ashes from incineration of Plastics,
kg 0,06
process per kg ashes and residues (kg)
Landfilling of ashes from incineration of
Polyethylene (PE), process per kg ashes and kg 0,01
residues (kg)
Landfilling of ashes from incineration of
Polyethylene terephthalate (PET), process per kg kg 0,00
ashes and residues (kg)
Landfilling of ashes from incineration of
Polyoxymethylene (POM), process per kg ashes kg 0,00
and residues (kg)
Landfilling of ashes from incineration of
Polypropylene (PP), process per kg ashes and kg 0,00
residues (kg)
Landfilling of ashes from incineration of
Polyvinylchloride (PVC), process per kg ashes and kg 0,02
residues (kg)
Landfilling of ashes from incineration of Rubber,
kg 0,06
municipal incineration with fly ash extraction (kg)
Landfilling of ashes from incineration per kg
kg 1,62
Hazardous waste, from incineration (kg)
Landfilling of ashes from incineration per kg
plastic, industrial electronics, From municipal kg 0,08
incineration with fly ash extraction (kg)
Substitution of primary steel with net scrap (kg) kg 0,05
Waste treatment per kg Brass slag, to landfill, kg 0,07
residual material landfill (kg)
Waste treatment per kg Copper slag, to landfill,
kg 0,39
residual material landfill (kg)
Waste, aluminium, to landfill (kg) kg 1,89
Waste, hazardous waste, to landfill (kg) kg 8,56
Waste, mineral wool, to landfil (kg) kg 10,96
Waste, plastic, mixture, to landfill (kg) kg 3,53
Waste, scrap steel, to landfill (kg) kg 26,32
Benefits and loads beyond the system
Unit Value
boundaries (D)
Substitution of electricity (MJ) MJ 4,38
Substitution of primary aluminium with net scrap
kg 25,13
(kg)
Substitution of primary Brass with net scrap (kg) kg 0,32
Substitution of primary copper with net scrap (kg) kg 2,56
Substitution of primary steel with net scrap (kg) kg 57,91
Substitution of thermal energy, district heating
MJ 66,24
(MJ)
7 / 13
LCA: Results
The LCA results are presented below for the declared unit defined on page 2 of the EPD document.
Environmental impact
Indicator Unit A1-A3 A4 C1 C2 C3 C4 D
GWP-total kg CO2 -eq 3,00E+03 5,13E+01 4,74E-01 3,21E+00 6,04E+01 5,47E+00 -3,00E+02
GWP-fossil kg CO2 -eq 2,96E+03 5,13E+01 4,74E-01 3,20E+00 6,03E+01 5,45E+00 -2,95E+02
GWP-biogenic kg CO2 -eq 3,11E+01 2,12E-02 8,88E-05 1,33E-03 8,90E-02 5,72E-03 -1,10E+00
GWP-luluc kg CO2 -eq 7,18E+00 1,82E-02 3,73E-05 1,14E-03 6,06E-03 1,71E-02 -4,29E+00
ODP kg CFC11 -eq 2,95E-04 1,16E-05 1,02E-07 7,26E-07 2,36E-06 3,30E-07 -2,80E-02
AP mol H+ -eq 2,51E+01 1,47E-01 4,96E-03 9,21E-03 4,15E-02 1,62E-02 -2,99E+00
EP-FreshWater kg P -eq 2,21E-01 4,10E-04 1,72E-06 2,56E-05 5,00E-04 1,16E-04 -2,05E-02
EP-Marine kg N -eq 3,12E+00 2,92E-02 2,19E-03 1,82E-03 1,14E-02 4,30E-03 -3,06E-01
EP-Terrestial mol N -eq 6,25E+01 3,26E-01 2,40E-02 2,04E-02 1,23E-01 4,27E-02 -3,53E+00
POCP kg NMVOC -eq 1,13E+01 1,25E-01 6,60E-03 7,81E-03 3,24E-02 1,58E-02 -1,23E+00
ADP-minerals&metals1 kg Sb -eq 1,43E+00 1,42E-03 7,27E-07 8,85E-05 8,07E-05 2,34E-05 -1,48E-02
ADP-fossil1 MJ 4,25E+04 7,75E+02 6,52E+00 4,84E+01 9,66E+01 4,05E+01 -3,45E+03
WDP1 m3 2,61E+05 7,50E+02 1,39E+00 4,69E+01 3,53E+02 1,66E+02 -1,24E+05
GWP-total = Global Warming Potential total; GWP-fossil = Global Warming Potential fossil fuels; GWP-biogenic = Global Warming Potential biogenic; GWP-luluc =
Global Warming Potential land use and land use change; ODP = Depletion potential of the stratospheric ozone layer; AP = Acidification potential, Accumulated
Exceedance; EP-freshwater = Eutrophication potential, fraction of nutrients reaching freshwater end compartment: EP-marine = Eutrophication potential, fraction of
nutrients reaching marine end compartment; EP-terrestrial = Eutrophication potential, Accumulated Exceedance; POCP = Formation potential of tropospheric ozone;
ADP-minerals&metals = Abiotic depletion potential for non-fossil resources; ADP-fossil = Abiotic depletion for fossil resources potential; WDP = Water (user)
deprivation potential, deprivation-weighted water consumption
"Reading example: 9,0 E-03 = 9,0*10-3 = 0,009"
*INA Indicator Not Assessed
1. The results of this environmental impact indicator shall be used with care as the uncertainties on these results are high or as there is limited experienced with the
indicator
Remarks to environmental impacts
8 / 13
Additional environmental impact indicators
Indicator Unit A1-A3 A4 C1 C2 C3 C4 D
PM Disease incidence 2,10E-04 3,14E-06 1,31E-07 1,96E-07 5,08E-07 2,49E-07 -2,34E-05
IRP2 kgBq U235 -eq 1,70E+02 3,39E+00 2,79E-02 2,12E-01 4,25E-01 1,26E-01 -1,23E+01
ETP-fw1 CTUe 1,33E+05 5,75E+02 3,56E+00 3,59E+01 5,06E+02 1,31E+03 -1,76E+04
HTP-c1 CTUh 1,02E-05 0,00E+00 0,00E+00 0,00E+00 2,14E-08 1,97E-08 -1,02E-06
HTP-nc1 CTUh 1,61E-04 6,28E-07 3,23E-09 3,92E-08 3,99E-07 8,41E-07 -1,29E-05
SQP1 dimensionless 1,78E+04 5,42E+02 8,27E-01 3,39E+01 3,71E+01 8,76E+01 -2,36E+02
PM = Particulate Matter emissions; IRP = Ionizing radiation – human health; ETP-fw = Eco toxicity – freshwater; HTP-c = Human toxicity – cancer effects; HTP-nc =
Human toxicity – non cancer effects; SQP = Potential Soil Quality Index (dimensionless)
"Reading example: 9,0 E-03 = 9,0*10-3 = 0,009"
*INA Indicator Not Assessed
1. The results of this environmental impact indicator shall be used with care as the uncertainties on these results are high or as there is limited experienced with the
indicator
2. This impact category deals mainly with the eventual impact of low dose ionizing radiation on human health of the nuclear fuel cycle. It does not consider effects due
to possible nuclear accidents, occupational exposure nor due to radioactive waste disposal in underground facilities. Potential ionizing radiation from the soil, from
radon and from some construction materials is also not measured by this indicator.
9 / 13
Resource use
Indicator Unit A1-A3 A4 C1 C2 C3 C4 D
PERE MJ 5,08E+03 1,11E+01 3,53E-02 6,93E-01 1,56E+01 8,44E+00 -1,13E+03
PERM MJ 6,21E-02 0,00E+00 0,00E+00 0,00E+00 -6,21E-02 0,00E+00 0,00E+00
PERT MJ 5,50E+03 1,11E+01 3,53E-02 6,93E-01 1,55E+01 8,44E+00 -1,13E+03
PENRE MJ 4,22E+04 7,75E+02 6,52E+00 4,84E+01 9,67E+01 4,05E+01 -3,45E+03
PENRM MJ 2,98E+02 0,00E+00 0,00E+00 0,00E+00 -2,60E+02 0,00E+00 0,00E+00
PENRT MJ 4,26E+04 7,75E+02 6,52E+00 4,84E+01 -1,64E+02 4,05E+01 -3,45E+03
SM kg 2,31E+02 0,00E+00 3,20E-03 0,00E+00 1,30E-05 1,86E-01 1,69E+00
RSF MJ 1,28E+02 3,97E-01 8,68E-04 2,48E-02 3,47E-01 4,81E-02 2,02E+00
NRSF MJ 5,79E+02 1,42E+00 1,28E-02 8,87E-02 -1,76E-02 1,74E+00 6,68E+01
FW m3 3,92E+01 8,29E-02 3,36E-04 5,18E-03 1,53E-01 7,57E-02 -5,97E+00
PERE = Use of renewable primary energy excluding renewable primary energy resources used as raw materials; PERM = Use of renewable primary energy resources used
as raw materials; PERT = Total use of renewable primary energy resources; PENRE = Use of non renewable primary energy excluding non-renewable primary energy
resources used as raw materials; PENRM = Use of non renewable primary energy resources used as raw materials; PENRT = Total use of non renewable primary energy
resources; SM = Use of secondary materials; RSF = Use of renewable secondary fuels; NRSF = Use of non-renewable secondary fuels; FW = Net use of fresh water
"Reading example: 9,0 E-03 = 9,0*10-3 = 0,009"
*INA Indicator Not Assessed
10 / 13
End of life - Waste
Indicator Unit A1-A3 A4 C1 C2 C3 C4 D
HWD kg 1,93E+01 4,00E-02 1,92E-04 2,50E-03 9,37E-02 9,29E+00 5,26E-01
NHWD kg 7,16E+02 3,77E+01 7,72E-03 2,36E+00 2,19E+01 5,85E+01 -9,45E+01
RWD kg 1,49E-01 5,28E-03 4,53E-05 3,30E-04 5,38E-05 6,60E-05 -1,16E-02
HWD = Hazardous waste disposed; NHWD = Non-hazardous waste disposed; RWD = Radioactive waste disposed
"Reading example: 9,0 E-03 = 9,0*10-3 = 0,009"
*INA Indicator Not Assessed
End of life - Output flow
Indicator Unit A1-A3 A4 C1 C2 C3 C4 D
CRU kg 0,00E+00 0,00E+00 0,00E+00 0,00E+00 0,00E+00 0,00E+00 0,00E+00
MFR kg 7,51E-01 0,00E+00 3,14E-03 0,00E+00 2,67E+02 7,53E-04 -8,41E-02
MER kg 2,99E-02 0,00E+00 9,75E-06 0,00E+00 1,15E+01 1,19E-05 -1,09E-02
EEE MJ 2,16E-02 0,00E+00 3,34E-05 0,00E+00 2,03E+01 5,34E-04 -3,33E-02
EET MJ 3,27E-01 0,00E+00 5,06E-04 0,00E+00 3,06E+02 8,08E-03 -5,03E-01
CRU = Components for re-use; MFR = Materials for recycling; MER = Materials for energy recovery; EEE = Exported energy electrical; EET = Exported energy thermal
"Reading example: 9,0 E-03 = 9,0*10-3 = 0,009"
*INA Indicator Not Assessed
Biogenic Carbon Content
Indicator Unit At the factory gate
Biogenic carbon content in product kg C 2,10E-03
Biogenic carbon content in accompanying packaging kg C 0,00E+00
Note: 1 kg biogenic carbon is equivalent to 44/12 kg CO2
11 / 13
Additional requirements
Greenhouse gas emissions from the use of electricity in the manufacturing phase
National production mix from import, low voltage (production of transmission lines, in addition to direct emissions and losses in grid) of applied
electricity for the manufacturing process (A3).
Electricity mix Data source Amount Unit
Electricity, market mix (kWh) - Germany ecoinvent 3.6 585,93 g CO2-eq/kWh
Dangerous substances
The product contains no substances on the REACH Candidate list at or above 100 ppm, 0,01 % by weight.
Indoor environment
Additional Environmental Information
Additional environmental impact indicators required in NPCR Part A for construction products
Indicator Unit A1-A3 A4 C1 C2 C3 C4 D
GWPIOBC kg CO2 -eq 2,99E+03 5,13E+01 4,74E-01 3,21E+00 6,04E+01 5,45E+00 -3,18E+02
GWP-IOBC: Global warming potential calculated according to the principle of instantaneous oxidation. In order to increase the transparency of biogenic carbon​
contribution to climate impact, the indicator GWP-IOBC is required as it declares climate impacts calculated according to the principle of instantaneous oxidation.​
GWP-IOBC is also referred to as GWP-GHG in context to Swedish public procurement legislation.
12 / 13
Bibliography
ISO 14025:2010 Environmental labels and declarations - Type III environmental declarations - Principles and procedures.
ISO 14044:2006 Environmental management - Life cycle assessment - Requirements and guidelines.
EN 15804:2012+A2:2019 Environmental product declaration - Core rules for the product category of construction products.
ISO 21930:2017 Sustainability in buildings and civil engineering works - Core rules for environmental product declarations of construction
products.
ecoinvent v3, Allocation, cut-off by classification, Swiss Centre of Life Cycle Inventories.
Iversen et al., (2021) eEPD v2021.09 Background information for EPD generator tool system verification, LCA.no Report number: 07.21
Graafland and Iversen (2022) EPD generator for NPCR 030 Ventilation components, Background information for EPD generator application and
LCA data, LCA.no report number: 12.22
NPCR Part A: Construction products and services. Ver. 2.0. April 2021, EPD-Norge.
NPCR 030 Part B for Ventilation components, Ver. 1.0, 18.05.2021, EPD Norway.
EN ISO 9001:2015 - Quality management systems.
EN ISO 14001:2015 - Environmental management systems.
EN ISO 50001:2018 - Energy management systems.
Program operator and publisher Phone: +47 23 08 80 00
The Norwegian EPD Foundation e-mail: post@epd-norge.no
Post Box 5250 Majorstuen, 0303 Oslo, Norway web: www.epd-norge.no
Owner of the declaration: Phone: +49 2845 2020
productsustainability-
TROX Group e-mail:
de@troxgroup.com
Heinrich-Trox-Platz 1, 47506 Neukirchen-Vluyn web: https://www.trox.de/en
Author of the Life Cycle Assessment Phone: +47 916 50 916
LCA.no AS e-mail: post@lca.no
Dokka 6B, 1671 web: www.lca.no
Developer of EPD generator Phone: +47 916 50 916
LCA.no AS e-mail: post@lca.no
Dokka 6B,1671 Kråkerøy web: www.lca.no
ECO Platform web: www.eco-platform.org
ECO Portal web: ECO Portal
13 / 13
