ENVIRONMENTAL PRODUCT DECLARATION
as per ISO 14025 and EN 15804+A2
Owner of the Declaration VJ Technology Ltd.
Publisher Institut Bauen und Umwelt e.V. (IBU)
Programme holder Institut Bauen und Umwelt e.V. (IBU)
Declaration number EPD-VJT-20240220-CBA1-EN
Issue date 14.09.2023
Valid to 13.09.2028
XPE440
VJ Technology Ltd.
www.ibu-epd.com | https://epd-online.com
General Information
VJ Technology Ltd. XPE440
Programme holder Owner of the declaration
IBU – Institut Bauen und Umwelt e.V. VJ Technology Ltd.
Hegelplatz 1 Brunswick Road 288
10117 Berlin TN23 1EN Ashford, Kent
Germany United Kingdom
Declaration number Declared product / declared unit
EPD-VJT-20240220-CBA1-EN The declared product is the two-component reaction resin mortar
"XPE440", manufactured by VJ Technology Ltd.. The declared unit is
based on 1 kg reaction resin product in the ratio at which the two
components must be mixed before use. The packaging is also included in
the calculation, since the product is sold by VJ Technology Ltd. with its
packaging. The declared unit is indicated in [kg].
This declaration is based on the product category rules: Scope:
Reaction resin products, 01.08.2021 This document covers the two-component reaction resin mortar "XPE440".
(PCR checked and approved by the SVR) To prepare the life cycle assessment [LCA], specific data were collected
from the VJ Technology Ltd. manufacturing facility. The assessment is
based on data from 2020 which correspond to the yearly average.
Issue date The owner of the declaration shall be liable for the underlying information
and evidence; the IBU shall not be liable with respect to manufacturer
14.09.2023
information, life cycle assessment data and evidences.
The EPD was created according to the specifications of EN 15804+A2. In
Valid to
the following, the standard will be simplified as EN 15804.
13.09.2028
Verification
The standard EN 15804 serves as the core PCR
Independent verification of the declaration and data according to ISO
14025:2011
internally X externally
Dipl.-Ing. Hans Peters
(Chairman of Institut Bauen und Umwelt e.V.)
Florian Pronold Angela Schindler,
(Managing Director Institut Bauen und Umwelt e.V.) (Independent verifier)
1 Environmental Product Declaration - VJ Technology Ltd. - XPE440
Product
+ 5°C 2880 min.
Product description/Product definition + 10°C 1680 min.
The declared product XPE440 is a two-component reaction + 15°C 1080 min.
resin mortar based on epoxy resin that is delivered in a two- + 20°C 720 min.
component plastic cartridge. The high-performance product is + 25°C 540 min.
applied through a static mixer using a manual, battery-operated + 35°C 360 min.
or pneumatic gun. It was specially developed for use in + 40°C 240 min.
securing threaded rods, rebar or internally threaded sleeves in
concrete. For more information, please refer to the relevant technical data
Marketing of the product in the EU/EFTA (except for sheet.
Switzerland) is governed by Regulation
(EU) No. 305/2011 (CPR). The product requires a Declaration Product performance values in accordance with the Declaration
of Performance subject to ETA-20/0202, ETA-20/0230 and of Performance with regard to its principal characteristics
ETA-24/0077 and CE marking. according to ETA-20/0202, ETA-20/0230 and ETA-24/0077.
Base materials/Ancillary materials
Application The declared product XPE440 is delivered as a two-component
The VJ Technology Injection System XPE440 is used to safely plastic cartridge and consists of a resin component and a
secure threaded rods, internally threaded sleeves and post- curing agent component in a 3:1 volume ratio. The mixing ratio
mortared rebar connections in cracked and uncracked C20/25 between the resin component and the curing agent component
to C50/60 concrete for a useful life of up to 100 years, and is is set automatically as the
suitable for installation in hammer-drilled (standard SDS and product is pushed out of the cartridge. Curing begins
hollow bit) and diamond-drilled holes at environmental immediately after the components are mixed.
temperatures between 0°C and 40°C. The VJ Technology
Injection System XPE440 has ETA assessments and ICC 1) "This product/article/at least one partial article contains
certifications, including seismic category C1 and C2 for substances in the ECHA candidate list of substances of very
anchoring from M8 to M30 and for rebar connections including high concern (SVHC) (17 January 2023) above a concentration
seismic conditions from 8mm to 40mm, and can be rated for fire of 0.1% by mass: no."
conditions.
2) "This product/article/at least one partial article contains other
Technical Data
CMR substances in categories 1A or 1B which are not on the
The following structural properties are relevant for the declared candidate list, exceeding 0.1 percentage by mass: no"
product XPE440 as delivered:
Construction Data 3) "Biocide products were added to this construction product or
it has been treated with biocide products (this then concerns a
Name Value Unit
treated product as defined by the (EU) Regulation on Biocidal
Density acc. to DIN 51757 for mixing the two
1.4 g/cm³ Products No. 528/2012): no"
components
Compressive strength acc. to DIN EN 196 Part 1 121.8N/mm² The product considered in this EPD contains individual
Flexural strength acc. to DIN EN 196 Part 1 66 N/mm² components in the following ranges:
Storage:
Resin component:
Store in a cool, dry and dark place; storage temperature: +5°C
Epoxy resin: 40 to 75% by weight
to +35°C
Mineral fillers: 30 to 40% by weight
Other components: < 5% by weight
Shelf life:
24 months in cartridge systems
Curing agent component:
Various polyamines: 40 to 50% by weight
Gel and working time:
Mineral fillers: 30 to 50% by weight
0°C 90 min.
Other components: < 5% by weight
+ 5°C 80 min.
+ 10°C 60 min.
Reference service life
+ 15°C 40 min.
The declared product XPE440 may be exposed to a wide range
+ 20°C 30 min.
of environmental conditions during the use phase. Its expected
+ 25°C 12 min.
reference service life depends on the specific installation
+ 35°C 8 min.
situation and on the product's resulting exposure. The main
+ 40 °C 8 min.
factors influencing service life
are weather conditions and mechanical and chemical stresses.
Curing time in dry substrate:
0°C 8640 min.
LCA: Calculation rules
XPE440. The declared unit is based on 1 kg reaction resin
Declared Unit product in the ratio at which the two components must be mixed
The product declared is a two-component reaction resin mortar before use. The mass mixing ratio between the resin
manufactured by VJ Technology Ltd. with the product name component and the curing agent component is 4:1 (volume
2 Environmental Product Declaration - VJ Technology Ltd. - XPE440
ratio 3:1). The packaging is also included in the calculation at
0.1435 kg per 1 kg of reaction resin product. The declared unit Figure 1 Information modules A1 to A3 of the product
data are presented in the table below:
Declared unit data
Name Value Unit
Declared unit 1 kg
Other declared units are allowed if the conversion is shown
transparently.
Figure 2 Information modules A1 to A3 of the packaging
System boundary
Type of EPD: Cradle to factory gate with options. The following Information modules C1 to C4 document
information modules are defined as system boundaries in this deconstruction/demolition for removal from the building,
study: transport to waste disposal, waste processing and product
disposal. Reuse, recovery and recycling potential are
Production stage (A1–A3): documented in information module D.
• A1, Raw material extraction,
Geographic Representativeness
• A2, Transport to the manufacturer,
Land or region, in which the declared product system is
• A3, Manufacturing.
manufactured, used or handled at the end of the product´s
lifespan: Germany
End of life (C1-C4):
• C1, Deconstruction/demolition,
• C2, Transport, Comparability
• C3, Waste processing, Basically, a comparison or an evaluation of EPD data is only
• C4, Disposal. possible if all the data sets to be compared were created
according to EN 15804 and the building context, respectively
Reuse, recovery and recycling potential (D) the product-specific characteristics of performance, are taken
into account.
To precisely determine the indicators and environmental The background datasets from the LCA for Experts and
impacts of the declared unit, a total of 8 information modules ecoinvent 3.9.1 databases, which this study also draws on, are
are considered. The information modules A1 to A3 describe the documented at the following site (Sphera). 2023.1
material provision, the transport to the production site, as well http://www.gabi-software.com/deutsch/index/ (ecoinvent 3.9.1).
as the production processes of the product itself. http://ecoquery.ecoinvent.org/3.9.1/cutoff/search
The precursor products are sourced from Germany. Transport
is exclusively done by truck. The following process diagrams
illustrate the underlying production process.
LCA: Scenarios and additional technical information
Name Value Unit
Characteristic product properties of biogenic carbon
Packaging PP 0.1188 kg
No renewable raw materials are used in the product or the
Packaging PA6 0.0082 kg
packaging. The biogenic carbon value is therefore reported as
zero. Packaging PE-LD 0.0165 kg
Packaging per declared unit End of Life (C1–C4)
The product is demolished by using an electric chisel. The
electrical energy consumption for this tool is estimated at 0.05
3 Environmental Product Declaration - VJ Technology Ltd. - XPE440
MJ for the declared unit. The power consumption is calculated
Reuse, recovery and recycling potential (D), relevant
using a European energy mix. Construcion waste is transported
scenario specifications
200 km by truck to a waste treatment facility. At the waste
The product has no reuse, recovery or recycling potential.
treatment facility, the construction waste is shredded and then
Information module D is therefore declared and reported as
disposed in a landfill.
zero.
Name Value Unit
Name Value Unit
Collected as mixed construction waste 1 kg
Reuse, recovery and recycling potential 0 kg
Shredding 1 kg
Disposal in landfill 1 kg
4 Environmental Product Declaration - VJ Technology Ltd. - XPE440
LCA: Results
The results in this calculation refer to the characterisation factors EN 15840+A2/EF 3.1.
DESCRIPTION OF THE SYSTEM BOUNDARY (X = INCLUDED IN LCA; MND = MODULE OR INDICATOR NOT DECLARED; MNR
= MODULE NOT RELEVANT)
Benefits and
Construction loads beyond
Product stage Use stage End of life stage
process stage the system
boundaries
la ire ta m w a Ry lp p u s tro p s n a rT g n iru tc a fu n a M e h t m o rf tro p s n a rTe tis e h t o t e ta g y lb m e s s A e s U e c n a n e tn ia M ria p e R tn e m e c a lp e R tn e m h s ib ru fe R y g re n e la n o ita re p Oe s u re ta w la n o ita re p Oe s u n o itc u rts n o c -e Dn o itilo m e d tro p s n a rT g n is s e c o rp e ts a W la s o p s iD -e s u e R-y re v o c e R-g n ilc y c e Rla itn e to p
A1 A2 A3 A4 A5 B1 B2 B3 B4 B5 B6 B7 C1 C2 C3 C4 D
X X X MND MND MND MND MNR MNR MNR MND MND X X X X X
RESULTS OF THE LCA - ENVIRONMENTAL IMPACT according to EN 15804+A2: 1 kg XPE440
Parameter Unit A1-A3 C1 C2 C3 C4 D
Global Warming Potential total (GWP-total) kg CO 2 eq 4.1E+00 4.58E-03 1.75E-02 2.58E-03 1.46E-02 0
Global Warming Potential fossil fuels (GWP-fossil) kg CO 2 eq 3.97E+00 4.53E-03 1.73E-02 2.56E-03 1.46E-02 0
Global Warming Potential biogenic (GWP-biogenic) kg CO 2 eq 1.26E-01 4.91E-05 0 0 0 0
Global Warming Potential luluc (GWP-luluc) kg CO 2 eq 8.91E-04 4.87E-07 1.58E-04 1.92E-05 4.53E-05 0
Depletion potential of the stratospheric ozone layer (ODP) kg CFC11 eq 2.19E-10 8.27E-14 1.49E-15 4.28E-15 3.71E-14 0
Acidification potential of land and water (AP) mol H+ eq 5.13E-03 9.57E-06 6.48E-05 1.34E-05 1.03E-04 0
Eutrophication potential aquatic freshwater (EP-freshwater) kg P eq 2.24E-05 1.67E-08 6.21E-08 8.71E-09 2.93E-08 0
Eutrophication potential aquatic marine (EP-marine) kg N eq 1.76E-03 2.29E-06 3.03E-05 6.13E-06 2.67E-05 0
Eutrophication potential terrestrial (EP-terrestrial) mol N eq 1.89E-02 2.39E-05 3.39E-04 6.77E-05 2.94E-04 0
Formation potential of tropospheric ozone photochemical oxidants kg NMVOC
5.94E-03 6.11E-06 5.84E-05 1.66E-05 8.06E-05 0
(POCP) eq
Abiotic depletion potential for non fossil resources (ADPE) kg Sb eq 2.08E-07 6.95E-10 1.1E-09 2.74E-09 6.72E-10 0
Abiotic depletion potential for fossil resources (ADPF) MJ 8.8E+01 9.43E-02 2.32E-01 5.04E-02 1.94E-01 0
m3 world eq
Water use (WDP) 1.21E-01 9.98E-04 1.96E-04 4.98E-04 1.6E-03 0
deprived
RESULTS OF THE LCA - INDICATORS TO DESCRIBE RESOURCE USE according to EN 15804+A2: 1 kg XPE440
Parameter Unit A1-A3 C1 C2 C3 C4 D
Renewable primary energy as energy carrier (PERE) MJ 8.76E+00 5.64E-02 1.64E-02 4.68E-03 3.16E-02 0
Renewable primary energy resources as material utilization
MJ 0 0 0 0 0 0
(PERM)
Total use of renewable primary energy resources (PERT) MJ 8.76E+00 5.64E-02 1.64E-02 4.68E-03 3.16E-02 0
Non renewable primary energy as energy carrier (PENRE) MJ 6.69E+01 9.43E-02 2.32E-01 5.05E-02 1.94E-01 0
Non renewable primary energy as material utilization (PENRM) MJ 2.11E+01 0 0 0 0 0
Total use of non renewable primary energy resources (PENRT) MJ 8.81E+01 9.43E-02 2.32E-01 5.05E-02 1.94E-01 0
Use of secondary material (SM) kg 0 0 0 0 0 0
Use of renewable secondary fuels (RSF) MJ 0 0 0 0 0 0
Use of non renewable secondary fuels (NRSF) MJ 0 0 0 0 0 0
Use of net fresh water (FW) m3 1.18E-02 4.55E-05 1.81E-05 1.44E-05 4.9E-05 0
RESULTS OF THE LCA – WASTE CATEGORIES AND OUTPUT FLOWS according to EN 15804+A2:
1 kg XPE440
Parameter Unit A1-A3 C1 C2 C3 C4 D
Hazardous waste disposed (HWD) kg 7.4E-09 7.38E-12 8.59E-13 1.31E-13 4.23E-12 0
Non hazardous waste disposed (NHWD) kg 6.94E-02 6.91E-05 3.35E-05 1.33E-05 9.71E-01 0
Radioactive waste disposed (RWD) kg 1.31E-03 1.5E-05 3E-07 6.77E-07 2.21E-06 0
Components for re-use (CRU) kg 0 0 0 0 0 0
Materials for recycling (MFR) kg 0 0 0 0 0 0
Materials for energy recovery (MER) kg 0 0 0 0 0 0
Exported electrical energy (EEE) MJ 0 0 0 0 0 0
Exported thermal energy (EET) MJ 0 0 0 0 0 0
RESULTS OF THE LCA – additional impact categories according to EN 15804+A2-optional:
1 kg XPE440
Parameter Unit A1-A3 C1 C2 C3 C4 D
Disease
Incidence of disease due to PM emissions (PM) ND ND ND ND ND ND
incidence
Human exposure efficiency relative to U235 (IR) kBq U235 eq ND ND ND ND ND ND
Comparative toxic unit for ecosystems (ETP-fw) CTUe ND ND ND ND ND ND
Comparative toxic unit for humans (carcinogenic) (HTP-c) CTUh ND ND ND ND ND ND
5 Environmental Product Declaration - VJ Technology Ltd. - XPE440
Comparative toxic unit for humans (noncarcinogenic) (HTP-nc) CTUh ND ND ND ND ND ND
Soil quality index (SQP) SQP ND ND ND ND ND ND
Disclaimer 2 - applies to the following indicators: 'Abiotic shortage potential - non-fossil resources', 'Abiotic shortage potential - fossil
fuels', 'Water deprivation potential (users)', 'Potential comparative toxic unit for ecosystems', 'Potential comparative toxic unit for human
health - carcinogenic effects', 'Potential comparative toxic unit for human health - non-carcinogenic effects', 'Potential soil quality index'.
The results of this environmental impact indicator shall be used with care, as the uncertainties of the results are high and as there is
limited experience with the indicator.
References
DIN 51757 http://www.ecoinvent.org
DIN 51757:2011-01 (26 May 2023)
Testing of mineral oils and related materials - Determination of
density. ETA-20/0202
European Technical Assessment
EN 196
DIN EN 196-1:2016-11 ETA-20/0230
Methods of testing cement - Part 1: Determination of strength. European Technical Assessment
EN 15804 ETA-24/0077
EN 15804+A2:2019+AC:2021, Sustainability of construction European Technical Assessment
works - Environmental product declarations - Core rules for the
product category of construction products. IBU 2021
Institut Bauen und Umwelt e.V.: General guidance for the EPD
EN/TR 15941 programme of the Institut Bauen und Umwelt e.V., Version 2.0,
CEN/TR 15941:2010-03: Sustainability of construction works - Berlin: Institut Bauen und Umwelt e.V., 2021. www.ibu-epd.com
Environmental product declarations - Methodology for selection
and use of generic data PCR Part A
Product Category Rules for Building-Related Products and
ISO 14025 Services - Calculation Rules for Life Cycle Assessment and
DIN EN ISO 14025:2011-10, Environmental labels and Requierements on the Project Report V1.3, Institut Bauen und
declarations - Type III Umwelt e.V., 08.2022
environmental declarations - Principles and procedures.
PCR: Reaction resin products
ISO 14044 Guidance-Texts for Building-Related Products and Services-
DIN EN ISO 14044:2006-10, Environmental management - Life PART B: Requirements on the Environmental Product
cycle assessment - Requirements and guidelines. Declarations for Reaction Resin Products,1 August 2021
Further references Sphera
LCA for Experts: 2023.1
ECHA candidates list Leinfelden-Echterdingen; Sphera
https://echa.europa.eu/de/candiate-list-substances-in-articles Solution GmbH (Ed.)
http://www. gabi-software.com/deutsch/index/
ECHA list (26 May 2023)
https://echa.europa.eu/de/candiate-list-table
Regulation (EU) No. 305/2011 (CPR)
ecoinvent 3.9.1
Background database: ecoinvent 3.9.1 Ziirich: ecoinvent (Ed.) Regulation (EU) No. 528/2012 (Biocidal Products Regulation)
6 Environmental Product Declaration - VJ Technology Ltd. - XPE440
Publisher
Institut Bauen und Umwelt e.V. +49 (0)30 3087748- 0
Hegelplatz 1 info@ibu-epd.com
10117 Berlin www.ibu-epd.com
Germany
Programme holder
Institut Bauen und Umwelt e.V. +49 (0)30 3087748- 0
Hegelplatz 1 info@ibu-epd.com
10117 Berlin www.ibu-epd.com
Germany
Author of the Life Cycle Assessment
FIT-Umwelttechnik GmbH 05362 72 69 474
Westerstr. 13 bertram@fit-umwelttechnik.de
38442 Wolfsburg www.fit-umwelttechnik.com
Germany
Owner of the Declaration
VJ Technology Ltd. +44 01233 637695
Brunswick Road 288 technical@vjtechnology.com
TN23 1EN Ashford, Kent www.vjtechnology.com
United Kingdom
7 Environmental Product Declaration - VJ Technology Ltd. - XPE440
