Applicant's logo]
DAPH S E P D
ABITAT YSTEM NVIRONMENTAL RODUCT ECLARATION
www.daphabitat.pt [in accordance with ISO 14025, EN 15804:2012+A2:2019 and EN 15942]
Declaration number: DAP 001:2024
PORTLAND CLINKER MACEIRA-LIZ PLANT
Issue date: 25/03/2024 Expiry date: 24/03/2029
SECIL – Companhia Geral de Cal e Cimento, S.A.
Version 1.4.1 Ed. March 2024
Index
1. GENERAL INFORMATION.................................................................................................................. 1
1.1. The DAPHabitat System ............................................................................................................................... 1
1.2. EPD Owner ................................................................................................................................................... 1
1.3. Information concerning the EPD .................................................................................................................. 2
1.4. Demonstration of the verification ............................................................................................................... 2
1.5. EPD Registration .......................................................................................................................................... 2
1.6. PCR (product category rules) basic model ................................................................................................... 3
1.7. Relevant c-PCR (Complementary product category rules) .......................................................................... 3
1.8. Information concerning the product/product class ..................................................................................... 4
1.9. Calculation rules of the LCA ......................................................................................................................... 4
1.10. Use of average environmental performance ............................................................................................... 5
1.11. Technical information for Reference Service Life (RSL) ............................................................................... 5
1.12. Flow diagram of input and output of the processes .................................................................................... 6
2. CORE ENVIRONMENTAL IMPACT INDICATORS ................................................................................ 7
2.1. Description of the system boundaries ......................................................................................................... 7
2.1.1. Justification for exemption of C1, C2, C3, C4 and D modules from declaration .......................................... 8
2.2. Core environmental impact indicators ........................................................................................................ 9
2.3. Additional environmental impact indicators ............................................................................................. 10
2.4. Indicators describing the utilisation of resources ...................................................................................... 11
2.5. Other environmental information describing different waste categories ................................................. 11
2.6. Environmental information describing output flows ................................................................................. 12
2.7. Information describing the biogenic carbon content at the fcatory gate .................................................. 12
3. REFERENCES ................................................................................................................................... 13
DAPHabitat System
iii
1. GENERAL INFORMATION
1.1. The DAPHabitat System
Platform for Sustainable Construction Association
Identification of the programme
www.clusterhabitat.pt
operator:
geral@clusterhabitat.pt
Departamento Engenharia Civil
Address: Universidade de Aveiro
3810-193 Aveiro
Email address: deptecnico@clusterhabitat.pt
Telephone number: (+351) 234 401 576
Website: www.daphabitat.pt
Logo:
1.2. EPD Owner
Owner’s name: SECIL – Companhia Geral de Cal e Cimento, S.A.
Address (production site): Rua da Sismaria, 16, Zona Industrial
2415-809 Marrazes
Address (head office):
Fábrica Maceira-Liz
2405-019, Maceira-Leiria
Telephone number: (+351) 217 927 100
Email address: apoiotecnico@secil.pt
Website: https://www.secil.pt/
Logo:
Information on management NP EN ISO 9001 – Quality Management System
NP ISO 14001 – Environmental Management System
systems in place:
ISO 45001 – Health and Safety Management System
EMAS | Eco-Management Audit Scheme
Specific aspects of CAE (economic activity code) 23510 – Manufacture of cement
production:
Organisation’s
Commitments made by SECIL as part of its Environmental Responsibility and Protection
environmental policy: policy:
• To ensure a responsible performance standard that makes using natural
resources compatible with the maintenance and development of the ecosystems
in which the company operates.
• To mitigate the impacts of its actions, through the adoption of the best
technologies and best practices available and the appropriate training of its
employees.
• To promote biodiversity in the territories under its management. To reduce the
carbon impact of its activity, including by promoting the use of secondary raw
materials and alternative fuels.
To provide the public with regular data on its environmental performance.
DAPHabitat System
1
1.3. Information concerning the EPD
Authors: Paula Quinteiro
Secil - Companhia Geral de Cal e Cimento, S.A.
Address: Universidade de Aveiro, Campus Universitário de Santiago, 3810-193 Aveiro,
Portugal
Telephone: 234 370 200
Authors’ contact:
E-mail: p.sofia@ua.pt
Address: Estrada do Outão s/n, 2901-864 Setúbal, Portugal
E-mail: info.pssg@secil.pt
Issue date: 25/03/2024
Registration date: 12/04/2024
Registration number: DAP 001:2024
Valid until: 24/03/2029
Representativeness of the EPD EDP of one (1) product class, produced in one (1) industrial unit, belonging to one (1)
(location, product, group of single producer (Secil - Companhia Geral de Cal e Cimento, S.A.)
producers):
Where to find product
https://www.secil.pt
information:
EPD type Cradle-to-gate EPD (A1-A3)
1.4. Demonstration of the verification
Independent external verification in accordance with the NP ISO 14025:2010 and EN 15804:2012+A2:2019 standards
Certification Body Verifier(s)
(CERTIF – Associação para a Certificação) (Marisa Almeida | José Dinis Silvestre)
1.5. EPD Registration
Registration Programme Operator
(Platform for Sustainable Construction)
DAPHabitat System
2
1.6. PCR (product category rules) basic model
Name: Base PCR model for construction products and services
Issue date: Edition August 2023
Database registration number: RCP-mb001
Version: Version 2.3
Identification and contact details of the Marisa Almeida | marisa@ctcv.pt
coordinator(s): Luís Arroja | arroja@ua.pt
José Dinis Silvestre | jose.silvestre@ist.utl.pt
Marisa Almeida | marisa@ctcv.pt
Identification and contact details of the
Luís Arroja | arroja@ua.pt
authors: José Silvestre | jds@civil.ist.utl.pt
Fausto Freire
Cristina Rocha
Ana Paula Duarte
Ana Cláudia Dias
Helena Gervásio
Victor Ferreira
Ricardo Mateus
António Baio Dias
Composition of the sector panel: -
Consultation period: 18/11/2015 - 18/01/2016
Valid until: 01/06/2027
The CEN EN 15804 standard serves as the basic product category rules (PCR).
1.7. Relevant c-PCR (Complementary product category rules)
EN 16908:2017+A1:2022 - Cement and building lime - Environmental product
Name:
declarations - Product category rules complementary to EN 15804
Issue date: March 2022
Database registration number: EN 16908:2017+A1:2022
Version: EN 16908:2017+A1, March 2022
Identification and contact details of the European Committee for Standardisation (CEN)
coordinator(s):
Identification and contact details of the -
authors:
Composition of the sector panel: -
Consultation period: -
Valid until: -
DAPHabitat System
3
1.8. Information concerning the product/product class
Product name: Clinker for Portland cement, or Portland clinker in short.
Product illustration:
Brief description of the product: The main raw materials used to produce Portland clinker are marl or clay and limestone,
which are extracted in quarries. Mining is carried out above ground, on plateaus, starting at
the highest level. The natural raw materials and secondary materials (e.g. correction
materials) are crushed, dosed and subjected to firing in which the physical-chemical
reactions (calcination) of the clinker process take place, to obtain Portland clinker. Portland
clinker is a fine granular material used as a binder in cement.
The clinker does not contain any substance included on the Candidate List of Substances of
Very High Concern (SVHC) above the limit for registration with the European Chemicals
Agency, i.e. above 0.1 per cent (m/m).
Main technical characteristics of the
Table 1: Technical characteristics and physical properties of Portland clinker.
product:
Designation Units Portland Clinker
Density g/cm3 Apparent 0.90 to 1.80
Solubility in water (T - 200C) g/l Mild (0.1 - 1.5)
pH (T = 200C; in water, water-solid -
11.0 - 13.5
ratio 1:2)
Melting point 0C Greater than 1250
Odour; Odour threshold - No odour threshold;
odourless
Description of the application/use of For the production of Portland cement and other hydraulic binders
the product:
Placing on the market/Rules for NP EN 197-1: Composition, specifications and conformity criteria for Ordinary cements
application on the market/Technical
product standards:
Quality control: Not applicable
Special delivery conditions: Not applicable
Components and substances to Not applicable
declare:
Information where explanatory Portland clinker is an intermediate material for physical integration into cement that is not
available for sale to the general public.
documents can be obtained: For detailed information on the product, please contact SECIL at info.pssg@secil.pt.
History of LCA studies: -
1.9. Calculation rules of the LCA
Functional unit: Not applicable
Declared unit: 1,000 kg of Portland clinker
System boundary: The system evaluated includes the A1-A3 module (product stage). A more detailed
description of the system boundary is given in Section 2.1.
Exclusion criteria: The LCA took into account the extraction and processing of natural raw materials, the
transport of secondary raw materials (including waste from other industries), the
production of auxiliary materials and the energy consumed in the manufacture of clinker.
Likewise, the waste management processes generated in the production of clinker (until the
end of waste status is reached) for which inventory data is available were considered. Bag
filters, the refractory lining of rotary kilns, lubricating oils, acetylene used in maintenance
operations (welding), sodium hypochlorite and sodium hydroxide used to treat the water
used in cooling towers were excluded from the system boundary, which individually
correspond to a mass of less than 1% of the total mass of inputs, and as a whole correspond
DAPHabitat System
4
to a mass of less than 5% of the total mass of inputs in module A1-A3. They are therefore
covered by the exclusion criteria defined in EN 16908:2017+A1 - Cement and building lime -
Environmental product declarations - Product category rules, namely their mass is less than
1% of the total mass of the inputs and does not exceed 5% of the total mass of the inputs of
each module. The LCA for Portland clinker also excluded energy and water consumption in
the administrative areas, as well as the production of wastewater and waste from these
areas. In addition, environmental loads associated with the construction and maintenance
of infrastructure and equipment (capital goods) were excluded.
Assumptions and limitations: The results of the environmental impacts and other indicators presented in this EPD refer to
the year 2021.
Quality and other characteristics of The quality of the inventory data was assessed taking into account the criteria of the PEF
(Product Environmental Footprint) category rules (section 5.6 of the guide, Menfredi et al.,
the information used in the LCA: 2012), as indicated in table E.2 (Data quality and criteria from the Product Environmental
Footprint Category Rules) of EN 15804:2012+A2:2019+AC and in the guide to the software
used, the GCCA EPD Tool for Cement and Concrete (V 4.0), and based on the
recommendations of the PCR documents - Base Model. The quality of the data was broadly
classified between reasonable and good on a 5-level qualitative scale from very bad to very
good, in line with the data quality requirements - temporal, geographical and technological.
The information on the production of Portland clinker is less than 5 years old, using mostly
primary data collected directly from SECIL - Maceira - Liz. Plant
For the operations associated with the Portland clinker manufacturing process, real data
specific to the production unit was used. The information for background processes not
provided by SECIL, and over which SECIL has no influence, was obtained from generic data in
the Ecoinvent database v3.5. These were selected to provide geographical and technological
coverage that fulfils the data quality criteria stipulated in Annex E of EN
15804:2012+A2:2019.
Electricity production was modelled in the GCCA with information obtained from SECIL’s
electricity producer and supplier.
Allocation rules: In addition to clinker production, bypass dust (by-product) is also produced, some of which
is sold and some of which is consumed internally. To determine the inputs and outputs
associated only with the production of clinker, the procedure for subdividing the unit
process was first adopted. Thus, only the operations associated with the production of the
product being analysed were taken into account, and operations exclusive to other products
were excluded. Then, for the operations included, an allocation procedure was applied
based on the mass of the different products produced.
The Portland clinker production process also involves multifunctionality associated with the
consumption of waste from other industries as secondary raw materials (e.g. shellac and
glaze, used refractories, boiler bottom ash, etc.) and secondary fuels (fuels derived from
waste, used tyre chips, etc.), so the environmental impacts associated with these raw
materials and fuels only concern the operations that take place from their transport to the
Maceira-LIZ plant. On the other hand, waste is produced that will later be recovered, for
which further processing has been considered up to the point at which it is expected to
reach end-of-waste status.
Software used for evaluation: GCCA EPD Tool for Cement and Concrete (V 4.0), International version.
Background database used for the Ecoinvent database version 3.5 published in December 2018; cut-off approach.
LCA:
Variability of the results of LCIA The composition of raw materials can also slightly affect the results of the LCIA.
The mix of fuels in the clinker kiln shows a variability of less than 10 per cent in the LCIA
results.
Comparability of construction EPD for construction products and services may not be comparable if they are not produced
products' EPD: following EN 15804 and EN 15942 and following the comparability conditions determined by
ISO 14025.
1.10. Use of average environmental performance
Not applicable
1.11. Technical information for Reference Service Life (RSL)
Not applicable
DAPHabitat System
5
1.12. Flow diagram of input and output of the processes
Figure 1: Flowchart of the Portland clinker manufacturing process.
DAPHabitat System
6
2. CORE ENVIRONMENTAL IMPACT INDICATORS
2.1. Description of the system boundaries
(✓= included; ND = module not declared)
PRODUCT CONSTRUCTION USE STAGE END OF LIFE STAGE ENVIRONMENTAL
STAGE PROCESS STAGE BENEFITS AND
BURDENS BEYOND
THE SYSTEM
BOUNDARY
s s g
e
c
o
n
o
n
ilc
s la ir e fot a ym lp w p ua Sr n o it a t r o p s n a r T g n ir u t c a fu n a M n o it a t r o p s n a r T r p n o it a lla ts n i d n a n o it c u r e s U e c n a n e tn ia M g n ir ia p e R tn e m e c a lp e R n o it a t ilib a h e R e s u y g r e n e la n o it a r e p O e s u r e t a w la n o it a r e p O itilo m e d d n a n o it c u r ts n o c n o it a t r o p s n a r T g n is s ee tc so a Wr p la s o p s iD y c e r la itn e t o p ,y r e v o c e r ,e
ts
n o C
e
D
s
u e R
A1 A2 A3 A4 A5 B1 B2 B3 B4 B5 B6 B7 C1 C2 C3 C4 D
✓ ✓ ✓ ND ND ND ND ND ND ND ND ND ND ND ND ND ND
The A1-A3 module (product stage) of Portland clinker takes into account the extraction and processing of primary (natural) raw materials, the
production of secondary raw materials, the transport of raw materials, additives, fuels and electricity to the production unit, the manufacture
of Portland clinker, as well as the processing of waste up to the end of its waste status or its final destination.
The raw material then enters the kiln, moving along the kiln due to its rotation and slight inclination, continuing to heat up and carrying out the
physical-chemical reactions of the clinker process at a temperature of up to 1450ºC, to ultimately obtain clinker. As firing is an energy-intensive
stage, primary fuels are used, i.e. fossil fuels, as well as secondary fuels (fuels derived from waste, e.g. used tyres, fluff and fuels derived from
waste).
The main raw materials used to produce Portland clinker are marl or clay and limestone, which are extracted in quarries. Mining is carried out
above ground, on plateaus, starting at the highest level.
Once the materials are extracted, they are in the form of blocks measuring up to 1m3, so it is necessary to reduce their size to a dimension
compatible with the transportation, storage and supply of the subsequent manufacturing phases; this operation is performed in the crusher.
After crushing, the natural raw materials are stored, which is combined with a pre-homogenisation function so that the various uniform
stockpiles.
This is followed by raw milling, in which the natural and secondary raw materials (materials derived from waste, e.g. foundry sands, ceramic
shards, calcium carbonate sludge, construction and demolition waste, used refractory bricks) are subjected to a drying, milling and
homogenising process. Once the proportion of raw materials has been defined, they are transported to mills where the "flour" or “raw”
material is produced, i.e. a finely ground mixture, in well-defined proportions, of all the natural and secondary raw materials. At this stage, the
raw material is dried using the heat contained in the exhaust gases from the rotary kilns.
This is followed by the preheating stage in which the raw material is extracted from the storage silos and fed into the preheating system
(cyclone tower), where it is heated by the exhaust gases resulting from the burning of the fuels in the rotary kiln.
From 1450ºC onwards, the clinker begins to cool, still inside the kiln, and is completed in the cooler, where counter-current air is introduced,
using this heated air as secondary firing air. In this way, there is a partial recovery of the clinker's thermal content to reduce energy
DAPHabitat System
7
consumption in the kilns. Particle matter emissions are controlled by dedusting systems and gas emissions into the air by automated control
systems for driving the furnaces. The firing phase produces a powder that comes from a bypass of the gaseous effluent to remove chlorides
from the raw material and fuels, which are then treated by a bag filter. This bypass powder is a by-product, partly sold and partly consumed
internally in cement production (used as a component in cement mills).
Finally, the clinker is stored for later use in the production of ordinary cement or other hydraulic binders. The transport of clinker to the mills or
for sale is carried out with bag filters to minimise diffuse dust emissions.
The LCA took into account the consumption of electricity, gases and lubricating oils, as well as internal movements in transport screens, for
example, the transport of crushed natural materials to the warehouse.
Portland clinker is produced 'dry', meaning that very little water is used during the production process. However, water is consumed through
evaporation in the cooling towers of the gases that go to the clinker kiln's bag filter. This water comes from our boreholes and requires
treatment with sodium hypochlorite and sodium chloride.
The diesel used for internal movements at Secil comes from a diesel refuelling station at the plant. Pollutant emissions to rainwater from the
hydrocarbon separators associated with the diesel refuelling station and the collection of oily water throughout the plant were therefore taken
into account. The diesel consumption of emergency generators was also taken into account to guarantee the normal operation of clinker
production processes in the event of a temporary power cut.
The transport and treatment of waste resulting from the clinker production process, such as waste containing hydrocarbons, was considered.
2.1.1. Justification for exemption of C1, C2, C3, C4 and D modules from declaration
Portland clinker, being an intermediate product, fulfils all the conditions required by EN 15804:2012+A2:2019+AC and EN 16908:2017+A1, to
consider the cradle-to-gate life cycle (A1-A3), namely:
▪ clinker is physically integrated into cement, which does not allow the physical separation of clinker and cement at the end of its life;
▪ the physical and chemical transformation process that clinker undergoes throughout its life cycle means that at the end of its life
this material is not identifiable;
▪ the clinker does not contain biogenic carbon.
DAPHabitat System
8
2.2. Core environmental impact indicators
Global Global Global warming Depletion
Global warming potential land potential of the Acidification
warming warming
potential biogenic; use and land use stratospheric potential;
potential total; potential fossil;
change; ozone layer;
GWP-biogenic AP
GWP-total GWP-fossil GWP-luluc ODP
Unit kg CO2 eq. kg CO2 eq. kg CO2 eq. kg CO2 eq. kg CFC 11 eq. mol H+ eq.
A1-A3 Module
8,29E+02 8,29E+02 4,51E-02 4,76E-02 1,25-05 1,83E+00
KEY:
Product Stage
Units expressed per declared unit (1000 kg Portland clinker).
Abiotic
Abiotic
depletion
Eutrophication Formation depletion
Eutrophication Eutrophicatio potential for Water (user)
potential potential of potential
potential n potential non-fossil deprivation
aquatic tropospheric for fossil
aquatic marine; terrestrial; resources potential;
freshwater; ozone; resources
potential
EP-marine EP-terrestrial ADP- WDP
EP-freshwater POCP
minerals&me
ADP-fossil
tals
m3 World eq.
Unit kg P eq. kg N eq. mol N eq. Kg COVNM eq. kg Sb eq. MJ, P.C.I
deprived
A1-A3 Module
1,60E-02 1,13E-03 6,45E+00 1,55E+00 1,26E-04 2,62E+03 1,50E+01
KEY:
Product Stage
Units expressed per declared unit (1000 kg Portland clinker).
The results obtained for the indicators "Non-fossil Abiotic Depletion Potential (ADP-minerals&metals)", "Fossil Abiotic Depletion Potential (ADP-fossil)" and
"Water Deprivation Potential (user) (WDP)" should be used with caution as the uncertainties associated with them are high or there is little experience with the
indicator.
DAPHabitat System
9
2.3. Additional environmental impact indicators
Potential
Potential Potential Potential Potential
Human
incidence of Comparative Comparative Toxic Comparative Toxic Potential soil
exposure
disease due to PM Toxic Unit for Unit for humans, Unit for humans, quality index
efficiency
emissions ecosystems cancer effects not cancer effects
relative to U235
SQP
PM ETP-fw HTP-c HTP-nc
IRP
Unit Disease incidence kBq U 235 eq. CTUe CTUh CTUh -
A1-A3 Module
4,33E-05 5,27E+03 7,52E+01 1,40E-06 4,25E-05 1,49E+03
KEY:
Product Stage
Units expressed per declared unit (1000 kg Portland clinker).
The impact indicator "Potential Human Exposure Efficiency in relation to U235 (IRP)" focuses mainly on the possible impact of a low dose of ionising radiation on
human health resulting from the nuclear fuel cycle. It does not take into account effects resulting from possible nuclear accidents, occupational exposure or the
disposal of radioactive waste in underground installations. Potential ionising radiation from soil, radon and some building materials is also not measured by this
indicator.
The results obtained for the indicators "Potential Comparative Toxic Unit for Ecosystems (ETP-fw)", “Potential Comparative Human Toxicity Unit, Carcinogenic
(HTP-c)", “Potential Comparative Human Toxicity Unit, Non-Carcinogenic (HTP-nc)" and "Soil Quality Potential Index (SQP)" should be used with caution as the
uncertainties associated with them are high or there is little experience with the indicator.
DAPHabitat System
10
2.4. Indicators describing the utilisation of resources
Primary energy
EPR RR TRR EPNR RNR TRNR
Unit MJ, P.C.I MJ, P.C.I MJ, P.C.I MJ, P.C.I MJ, P.C.I MJ, P.C.I
A1-A3 Module
1,84E+02 0,00E+00 1,84E+02 2,52E+03 0,00E+00 2,52E+03
KEY:
Product Stage
Units expressed per declared unit (1000 kg Portland clinker).
EPR = use of renewable primary energy excluding renewable primary energy resources used as raw materials; RR = use of renewable primary energy resources
used as raw materials; TRR = total use of renewable primary energy resources (EPR + RR); EPNR = use of non-renewable primary energy excluding non-
renewable primary energy resources used as raw materials; RNR = use of non-renewable primary energy resources used as raw materials; TRNR = total use of
non-renewable primary energy resources (EPRN + RNR)
Secondary material and fuel, and water use
Utilising the net value of
MS CSR CSNR
fresh water
Unit kg MJ, P.C.I MJ, P.C.I m3
A1-A3 Module
1,18E+02 6,18E+02 8,14E+02 2,95E-01
KEY:
Product Stage
Units expressed per declared unit (1000 kg Portland clinker).
MS = use of secondary material; CSR = use of renewable secondary fuels; CSNR = use of non-renewable secondary fuels; Fresh water = use of the net value of
fresh water.
2.5. Other environmental information describing different waste categories
Hazardous waste disposed Non-hazardous waste disposed Radioactive waste disposed
Unit kg kg kg
A1-A3 Module
5,66E-01 1,06E-02 0,00+00
KEY:
Product Stage
Units expressed per declared unit (1000 kg Portland clinker).
The characteristics that make waste hazardous are described in the applicable legislation in force, for example in the European Waste Framework Directive.
DAPHabitat System
11
2.6. Environmental information describing output flows
Materials for Exported energy
Components for Materials for
recycling
reuse energy recovery
Unit kg kg kg MJ
Modules A1-A3
0,00E+00 1,03E+00 4,07E-01 0,00E+00
KEY:
Product Stage
Units expressed per declared unit (1000 kg Portland clinker).
The characteristics that make waste hazardous are described in the applicable legislation in force, for example in the European Waste Framework Directive.
2.7. Information describing the biogenic carbon content at the fcatory gate
Biogenic carbon content* Units** Modules A1-A3 (results)
Biogenic carbon content in the product Kg C Not applicable
Biogenic carbon content in the packaging Kg C Not applicable
* 1 kg of biogenic carbon is equivalent to 44/12 kg of CO2
** This information may be omitted when the biogenic carbon content of the product or its packaging is less than 5 per cent of the mass of the
product or its packaging.
DAPHabitat System
12
3. REFERENCES
✓ GCCA (2023). GCCA Industry EPD Tool for cement and concrete (V4.0). Global Cement and Concrete Association
(GCCA) Quantis, Switzerland;
✓ DAPHabitat System General Instructions, Version 2.1, August 2023 (at www.daphabitat.pt);
✓ PCR - Base Model. Construction products and services. Following EN 15804:2012+A2:2019. DAPHabitat
System. Version 2.3, August 2023 (at www.daphabitat.pt);
✓ NP ISO 14025:2009 Environmental labelling and declarations - Type III environmental declarations - Principles
and procedures;
✓ EN 15804:2012+A2:2019+AC Sustainability of construction works - Environmental product declarations - Core
rules for the product category of construction products;
✓ EN 16908:2017+A1 - Cement and building lime - Environmental product declarations - Product category rules
complementary to EN 15804 European Committee for Standardisation;
✓ EN 15942:2021 Sustainability of construction works – Environmental product declarations – Communication
format business-to-business;
✓ Manfredi S., Allacker K., Chomkhamsri K., Pelletier N., Maia de Souza D. (2012). Product Environmental
Footprint (PEF) Guide. European Commission (EC), Joint Research Centre (JRC), Ispra, Italy;
✓ Secil (2023). Secil CO Manual. Monitoring, calculating and reporting CO emissions. Period 2021-2025. Version
2 2
06.
DAPHabitat System
13
