Logo of the EPD’s owner]
DAPHabitat System Environmental Product Declaration
www.daphabitat.pt [according to ISO 14025, EN 15804:2012+A2:2019 and EN 15942]
Declaration number: DAP 020:2024
UNWASHED AGGREGATES – ATOUGUIA QUARRY
ISSUE DATE: 20/12/2024 VALID UNTIL: 19/12/2029
SECIL AGREGADOS, S.A.
Version 1.4.1 Ed. March 2024
1
Index
1. GENERAL INFORMATION ................................................................................................................. 2
1.1. The DAPHAbitat System .............................................................................................................................. 2
1.2. EPD owner ................................................................................................................................................... 2
1.3. Information concerning the EPD ................................................................................................................. 3
1.4. Demonstration of the verification .............................................................................................................. 3
1.5. EPD Registration .......................................................................................................................................... 3
1.6. PCR (product category rules) basic model .................................................................................................. 4
1.7. Relevant c-PCR (Complementary product category rules) ......................................................................... 4
1.8. Information concerning the product/product class ................................................................................... 5
1.9. Calculation rules of the LCA ........................................................................................................................ 6
1.10. Use of average environmental performance ............................................................................................. 7
1.11. Technical information for Reference Service Life (RSL) ............................................................................. 7
1.12. Flow diagram of input and output of the processes .................................................................................. 8
2. CORE ENVIRONMENTAL IMPACT INDICATORS............................................................................... 9
2.1. Description of the system boundaries ........................................................................................................ 9
2.1.1. Justification for the exemption to declare modules C1, C2, C3, C4 and D............................................... 10
2.2. Core environmental impact indicators ..................................................................................................... 11
2.3. Additional environmental impact indicators ........................................................................................... 12
2.4. Indicators describing resource use ........................................................................................................... 13
2.5. Other environmental information describing different waste categories .............................................. 13
2.6. Environmental information describing output flows ............................................................................... 14
2.7. Information describing the biogenic carbon content at the factory gate ............................................... 14
3. SCENARIOS AND ADDITIONAL TECHNICAL INFORMATION .......................................................... 14
3.1. Scenario and technical information for module D ................................................................................... 14
3.2. Additional information on release of dangerous substances to indoor air, soil, and water during the
use stage ................................................................................................................................................................. 14
4. REFERENCES ................................................................................................................................... 15
DAPHabitat System 1
1. GENERAL INFORMATION
1.1. The DAPHAbitat System
Sustainable Construction Platform
Program operator: www.clusterhabitat.pt
geral@clusterhabitat.pt
Departamento Engenharia Civil
Address: Universidade de Aveiro
3810-193 Aveiro
Email address: deptecnico@clusterhabitat.pt
Telephone number: (+351) 234 401 576
Website: www.daphabitat.pt
Logo
1.2. EPD owner
Name of the owner: Secil Agregados, S.A.
Production site: Serra da Atouguia – 2580-079 Ota
Address (head office): Av. Eng. Duarte Pacheco 19, 7º – 1070-100 Lisboa - Portugal
Telephone: (+351) 217 927 100
E-mail: apoiotecnico@secil.pt
Website: https://www.secil.pt/
Logo:
Information concerning the
applicable management
NP EN ISO 9001 - Quality management systems
Systems:
Specific aspects regarding the
Main CAE: 08121 - Extraction of gravel, sand and crushed stone;
production: Secondary CAE: 08112 - Extraction of ornamental granite and similar stones
Commitments made by SECIL as part of its Environmental Responsibility and Protection policy:
To guarantee a standard of responsible action that reconciles the exploitation of natural resources with
Organization’s environmental the maintenance and development of the ecosystems in which it operates. Mitigate the impacts of its
policy: operations by adopting the best available technologies and best practices and by providing adequate
training for its employees. Promote biodiversity in the territories under its management. Reduce the
carbon impact of its activity, specifically by promoting the use of secondary raw materials and alternative
fuels. To make data on its environmental performance available to the public on a regular basis.
2 Sistema DAPHabitat
1.3. Information concerning the EPD
Authors:
c5Lab - Sustainable Construction Materials Association
Contact of the authors: Edifício Central Park, Rua Central Park 6 | 2795-242 LINDA-A-VELHA
Email: info@c5lab.pt
Issue date: 20/12/2024
Registration date: 03/01/2025
Registration number: DAP 020:2024
Valid until: 19/12/2029
Representativity of the EPD
(location, manufacturer,
EPD for unwashed aggregates produced at the Atouguia quarry belonging to Secil Agregados, S.A.
group of manufacturers):
Where to consult
https://www.secil.pt/
explanatory material:
Type of EPD:
Cradle-to-gate (A1-A3) EPD.
1.4. Demonstration of the verification
External independent verification, accordingly, with the standard ISO 14025:2010 and EN 15804:2012+A2:2019
Certification Body Verifier
(CERTIF – Associação para a Certificação) (Marisa Almeida)
1.5. EPD Registration
Programme operator
(Plataforma para a Construção Sustentável)
DAPHabitat System 3
1.6. PCR (product category rules) basic model
Name:
PCR: Basic module for construction products and services
Issue date:
Edition August 2023
Number of registrations on the data
RCP-mb001
base:
Version:
Version 2.3
Identification and contact of the Marisa Almeida | marisa@ctcv.pt
coordinator (s): Luís Arroja | arroja@ua.pt
José Dinis Silvestre | jose.silvestre@ist.utl.pt
Identification and contact of the Marisa Almeida | marisa@ctcv.pt
authors: Luís Arroja | arroja@ua.pt
José Silvestre | jds@civil.ist.utl.pt
Fausto Freire
Cristina Rocha
Ana Paula Duarte
Ana Cláudia Dias
Helena Gervásio
Victor Ferreira
Ricardo Mateus
António Baio Dias
Composition of the Sectorial Panel:
-
Consultation period:
18/11/2015 - 18/01/2016
Valid until:
01/06/2027
CEN standard EN 15804 serves as the core Product Category Rules (PCR)
1.7. Relevant c-PCR (Complementary product category rules)
Not Applicable.
4 Sistema DAPHabitat
1.8. Information concerning the product/product class
Identification of the
Agregados Não Lavados – Pedreira Atouguia (Unwashed Aggregates)
product:
Illustration of the
product:
Brief description of the Industrial aggregates are granular materials, of mineral origin and generally inert. They are used in different
product: construction products and their choice has a strong influence on the quality and behaviour of the end
products.
Main technical The Unwashed Aggregates product class comprises a set of 4 (four) products manufactured by Secil
characteristics of the Agregados, S.A. at the Atouguia Quarry and listed in Table 1.
product:
Table 1 - Product Technical Characteristics and Performance Declarations.
Granulometry Description
Product Performance Declaration (In Portuguese)
(mm)
Pó de Pedra 0/4 Fine material from rock crushing https://bit.ly/DOP1_Po_Pedra
Unwashed gravel of larger
Brita 3 16/32 https://bit.ly/DOP6_Brita_3
nominal size
Material used before any
1ª treatment, with an extensive https://bit.ly/DOP7_Tout-Venant_1ª
Tout- 0/32 particle size range
Venant
Similar to 1st class Tout-Venant,
2ª https://bit.ly/DOP8_Tout-Venant_2ª
but of lower quality
Enrocamento 90/250 Large-scale aggregates. https://bit.ly/DOP9_Enrocamento
Description of the Aggregates have specific properties suitable for civil engineering works and can be used in the manufacture
product’s of concrete, mortar and bituminous mixtures or used without any hydraulic or other binder and in hydraulic
application/use: protection or regulation works.
Placing on the market /
Table 2 - Technical Product Standards and Intended Uses.
Rules of application in
Product Technical Rules Intended uses
the market / Technical
rules of the product: Non-Bonded Materials: NP EN Typical use in non-bonded materials for
Pó de Pedra use in civil engineering and road
13242:2002+A1:2010;
construction.
Concrete– NP EN
12620:2002+A1:2008;
Use in:
• Concrete for buildings, roads and
Bituminous mixtures - other civil engineering work;
NP EN 12620:2002+A1:2008; • Bituminous mixtures and surface
Brita 3
NP EN 13043:2004; treatments for roads, airports and
NP EN 13043/AC:2010; other traffic areas;
NP EN 13043:2004 ERRATA 1:2018; • Unbound materials for use in civil
engineering and road construction.
Non-Bonded Materials – NP EN
13242:2002+A1:2010;
Non-Bonded Materials – NP EN Use in non-bonded materials for use in civil
Tout-Venant
13242:2002 + A1:2010; engineering and road construction.
Use in hydraulic protection or regulation
Enrocamento Rockfill – NP EN 13383-1:2010
works
Quality control: The Unwashed Aggregates produced comply with CE marking requirements and their quality is controlled in
compliance with Regulation (EU) No. 305/2011 of 9 March 2011.
DAPHabitat System 5
Special delivery Disturbances to the normal supply of unwashed aggregates due to unforeseeable circumstances or force
conditions: majeure, such as strikes, riots, equipment breakdowns and accidents and power cuts by the entities
responsible for supplying them, provided that they are not attributable to Secil Agregados, S.A., do not
constitute a breach of the supply contract and will therefore not give rise to the payment of any
compensation. When the aggregates are delivered to the site and before they are unloaded, the Customer
or its representative must check on the delivery note that the product corresponds to that requested.
Signing the delivery note implies confirmation of what it says.
Components and
Not Applicable.
substances to declare:
Where explanatory
material may be https://www.secil.pt/
obtained:
History of the LCA
Not Applicable.
studies:
1.9. Calculation rules of the LCA
Functional unit: Not Applicable.
Declared unit: 1 tonne of Unwashed Aggregates
System boundaries: Cradle-to-Gate EPD. From the extraction and processing of raw materials in the quarry to the product
dispatch procedure.
Criteria for the Processes that fulfil the exclusion criteria stipulated in EN 15804 of 1% use of primary energy (renewable
and non-renewable) and 1% of the inputs or outputs (in mass) of the process, not exceeding 5% of the total
exclusion: use of mass and energy in the production stage, A1-A3, were excluded from this EPD:
• Production of By-product ‘Detritos’ • Domestic effluents
• Production of By-product ‘Alvenaria’ • Absorbents and filter materials
• Equipment maintenance • Oil filters
• Office activity • Sieving Nets
• Acetylene • Other minor components
Assumption and The missing data refers to indicators that cannot be acquired on site, namely: dust emissions from quarry
activity; emissions from quarrying machinery, loading and blasting.
limitations This missing information was therefore extracted from generic processes available in the Ecoinvent 3.10
database. In addition, the 1st and 2nd category ‘Tout-Venant’ products go through the same processing
chain, and their environmental impact is assumed to be equivalent, as their differentiation is solely due to
the quality of the raw material. These products were therefore combined into a single product category
called ‘Tout-Venant’.
Quality and other The quality analysis was carried out based on the ‘UN Environmental Global guidance on LCA database
development’ in accordance with the criteria stipulated in Annex E of EN 15804:2012+A2:2019. The quality
characteristics about the of the data was categorised broadly between fair and very good on a 5-level qualitative scale from very
poor to very good. The information on aggregate production is 1 year old, using mostly primary data
information used in the
collected directly from the quarry's industrial statistics and is representative of the reality of production.
LCA:
Information for background processes not provided by the quarry, and over which Secil Agregados, S.A. has
no direct influence, was obtained using generic data from the Ecoinvent 3.10 database (updated in April
2024). This data was selected to provide geographical and technological coverage that fulfils the data
quality criteria stipulated in Annex E of EN 15804:2012+A2:2019.
Electricity production for the year 2023 was modelled using information obtained directly from the
regulator of energy production and electricity infrastructure in Portugal. The results obtained are robust.
The LCA was carried out using SimaPro 9.6.0.1 software.
Allocation rules: To avoid the allocation of co-products, the inventory and impact analyses were carried out individually for
each of the four products. However, mass allocation procedures are necessary for the consumption of
energy, fuel, other consumables and waste.
Knowing the power of each equipment and the total electricity consumption in the crushing, the
distribution of consumption by equipment was carried out. In the crushing operation, consumption was
distributed proportionally for each product, according to the power of the equipment used, the frequency
of its use and the share of production associated with each piece of equipment.
The distribution of lubricating oil consumption for each product was calculated in a similar way to electricity
consumption, using the power of the equipment used, the frequency of its use and the share of production
associated with each piece of equipment. Diesel consumption associated with the processes of blasting,
6 Sistema DAPHabitat
loading and transporting each product was determined from overall consumption, using the relative
production masses of each unit.
The generation of dry solid waste associated with each product was distributed proportionally to its
production.
Software used for the SimaPro 9.6.0.1 – PRé Sustainability
assessment:
Background database Ecoinvent Database v3.10 – Ecoinvent
used for the LCA:
Comparability of EPD for The EPD of construction products and services cannot be comparable in case they are not produced
according to EN 15804 and EN 15948 and according to the comparability conditions determined by ISO
construction products 14025.
1.10. Use of average environmental performance
The ‘Unwashed Aggregates’ class of products produced by Secil Agregados, S.A. at the Atouguia quarry, and used
as building materials, differ mainly in their granulometry, even though the raw material (limestone) and
production method (crushing and screening) are identical. To provide robust results and reduce errors associated
with the use of average values, the impacts of each of the unwashed aggregates are presented separately, thus
avoiding the use of average environmental performance for a series of products with different production stages
and final application
The average difference between the maximum and minimum values (for the core environmental impact
indicators) is around 9 per cent, with the greatest variability (41%) occurring only in one core environmental
impact category (Water Deprivation Potential). There are occasions when there are greater differences, but these
occur in optional impact categories or secondary indicators.
1.11. Technical information for Reference Service Life (RSL)
Not Applicable.
DAPHabitat System 7
1.12. Flow diagram of input and output of the processes
8 Sistema DAPHabitat
L
R o a d tra n s p o rtT
a n k e r lo rry
6 .5 6 k g k m
D ie s e lL
o a d in g a n d T ra n s p o
1 2 .1 4 M J
u b ric a tin g O il
Y
rt
A
U
g
n
1
g
w
r
T
Ne
a
o
F e e d e r In p
1 .1 2 t
o n - W a sg
a t e s P r
1 t
L i f e C y cs
h e d A g
1 t
n n e U n wA
g g r e g a
u t
h e do
d u
l e -
g r e g
a s ht
e s
c
a
e
t i o
t e
d
n
s
0 .0 1
L
E
T
P
B
E le c tric ityC
ru sh in g
X
D e b r is S e n t to D u m p s t
e g e n d ( P e r T o n n e o f A g g r e g a
n r o c a m e n t o : X = 0 .5 8 k W h ; Y = 0 .0 0
o u t -V e n a n t : X = 1 .6 6 k W h ; Y = 0 .0 0 7
ó d e P e d r a : X = 1 .7 5 k W h ; Y = 0 .0 0 7 p
r it a 3 : X = 1 .6 1 k W h ; Y = 0 .0 0 7 p .
t e s )
2 p .
p .
.
:
Figure 1: Simplified flowchart for the inventory of Unwashed Aggregates production.
2. CORE ENVIRONMENTAL IMPACT INDICATORS
2.1. Description of the system boundaries
(✓= included; ND = module not declared)
BENEFITS AND LOADS
CONSTRUCTION
PRODUCT STAGE USE STAGE END OF LIFE STAGE BEYOND THE SYSTEM
PROCESS STAGE
BOUNDARY
la
y lp p u s la ire ta m w a R tro p s n a rT g n iru tc a fu n a M tro p s n a rT s s e c o rp n o ita lla ts n i n o itc
u
e s U e c n a n e tn ia M ria p e R tn e m e c a lp e R tn e m h s ib ru fe R e s u y g re n e la n o ita re p O e s u re ta w la n o ita re p O n o itilo m e d ,s n o itc u rts n eo Dc - tro p s n a rT g n is s e c o rp e ts a W la s o p s iD
itn
e to p g n ilc y c e r ,y re v o c e r ,e es u
-
rts R
n
o
C
A1 A2 A3 A4 A5 B1 B2 B3 B4 B5 B6 B7 C1 C2 C3 C4 D
✓ ✓ ✓ ND ND ND ND ND ND ND ND ND ND ND ND ND ND
The system boundaries are circumscribed for the Product Stage, covering modules A1-A3. All aggregates produced
at the Atouguia quarry are produced as described in the following points:
Blasting
The first stage of aggregate production consists of blasting, which involves extracting large blocks of rock from the
exploration front. This process begins with the selection of the area to be blasted and subsequent drilling, followed
by the placement of explosives. The detonation of these explosives fragments the rock mass. After the explosion,
the area is cleared, and the explosive packaging is incinerated on site. If necessary, deforestation is carried out and
the removed land is stored for later landscaping.
Crushing and Screening
The material obtained from blasting is transported to the crushing area, where the first reduction in the size of the
rock blocks takes place. This process begins with the rock being deposited in a feeding system, where larger blocks
are reduced and sent to a screen that separates the smaller particles, known as ‘Detritos’ (Debris), from those
suitable for producing aggregates, which are taken to a primary impact crusher.
DAPHabitat System 9
This impact crusher is responsible for fragmenting the larger rocks, which are then passed on to a system of
additional screens that carry out a new particle size separation. The particles that are still larger than desired are
redirected to a secondary crusher (hammer mill) which carries out additional crushing, further reducing the
particle size. Subsequently, the material is again subjected to a screening process, where it is classified by particle
size, resulting in different types of aggregates, ready for commercialisation or for subsequent processes, such as
washing. There may be recirculation of material whose size is larger than intended after passing through the
crushers. This material is re-crushed until it reaches the required size.
2.1.1. Justification for the exemption to declare modules C1, C2, C3, C4 and D
Unwashed Aggregates from the SECIL-Atouguia quarry are intermediate construction products that are physically
integrated with other products (among others, cement and water in the case of their use in concrete products).
They can have different end uses, which are impossible to generalise. In addition, biogenic carbon is not present in
the product, so according to standard NP EN 15804:2012+A2:2019 only modules A1-A3 can be declared.
10 Sistema DAPHabitat
2.2. Core environmental impact indicators
Depletion
Global Global warming
Global warming Global warming potential of the
warming potential land use
potential fossil; potential biogenic; stratospheric Acidification
potential total; and land use change;
ozone layer; potential; AP
GWP-fossil GWP-biogenic
Modules A1-A3 GWP-total GWP-luluc ODP
Unit kg CO2 eq. kg CO2 eq. kg CO2 eq. kg CO2 eq. kg CFC 11 eq. mol H+ eq.
Enrocamento 1.95E+00 1.95E+00 -4.70E-03 4.41E-03 3.19E-08 7.11E-02
Tout-Venant 2.15E+00 2.14E+00 -2.98E-03 1.14E-02 3.68E-08 7.16E-02
Pó de Pedra 2.17E+00 2.16E+00 -2.83E-03 1.20E-02 3.72E-08 7.17E-02
Brita 3 2.14E+00 2.13E+00 -3.05E-03 1.11E-02 3.66E-08 7.16E-02
LEGEND:
Product stage
Eutrophication Abiotic Abiotic
Eutrophication Formation
p ao qt uen att ii ca l potential Eu ptr oo tp eh nic ta iati lo n potential of pod te ep nle tit aio l fn o r pod te ep nle tit aio l fn o r W dea pte rir
v
( au ts ioe nr)
freshwater; aquatic terrestrial; tropospheric non-fossil fossil potential;
marine; ozone; resources resources
potential
EP- EP-terrestrial WDP
EP-marine POCP ADP-
Modules A1-A3 freshwater minerals&metals ADP-fossil
m3 World eq.
Units kg P eq. kg N eq. mol N eq. Kg COVNM eq. kg Sb eq. MJ, P.C.I
deprived
Enrocamento 9.90E-05 2.40E-02 3.63E-01 7.27E-02 7.32E-07 2.32E+01 3.09E-01
Tout-Venant 1.07E-04 2.41E-02 3.65E-01 7.34E-02 7.43E-07 2.70E+01 5.09E-01
Pó de Pedra 1.08E-04 2.41E-02 3.65E-01 7.34E-02 7.44E-07 2.74E+01 5.26E-01
Brita 3 1.07E-04 2.41E-02 3.65E-01 7.34E-02 7.42E-07 2.69E+01 5.01E-01
LEGENDA:
Product stage
DAPHabitat System 11
2.3. Additional environmental impact indicators
Potential Potential
Potential Potential Potential
incidence of Human Comparative
Comparative Comparative Toxic Potential soil
disease due exposure Toxic Unit for
Toxic Unit for Unit for humans, quality index
to PM efficiency humans, not
ecosystems cancer effects
emissions relative to U235 cancer effects SQP
Modules A1-A3 PM IRP ETP-fw HTP-c HTP-nc
Disease
Unit kBq U 235 eq. CTUe CTUh CTUh -
incidence
Enrocamento 8.41E-07 4.66E-02 4.39E+01 2.35E-09 4.38E-09 9.17E+01
Tout-Venant 8.44E-07 1.06E-01 4.40E+01 2.41E-09 5.06E-09 9.47E+01
Pó de Pedra 8.45E-07 1.12E-01 4.40E+01 2.41E-09 5.12E-09 9.49E+01
Brita 3 8.44E-07 1.04E-01 4.40E+01 2.40E-09 5.04E-09 9.45E+01
LEGEND:
Product stage
12 Sistema DAPHabitat
2.4. Indicators describing resource use
Primary energy
Modules A1-A3 EPR RR TRR EPNR RNR TRNR
Unit MJ, P.C.I. MJ, P.C.I. MJ, P.C.I. MJ, P.C.I. MJ, P.C.I. MJ, P.C.I.
Enrocamento 2.28E+00 0.00E+00 2.28E+00 2.32E+01 0.00E+00 2.32E+01
Tout-Venant 5.53E+00 0.00E+00 5.53E+00 2.70E+01 0.00E+00 2.70E+01
Pó de Pedra 5.81E+00 0.00E+00 5.81E+00 2.74E+01 0.00E+00 2.74E+01
Brita 3 5.41E+00 0.00E+00 5.41E+00 2.69E+01 0.00E+00 2.69E+01
LEGEND:
Product stage
EPR = use of renewable primary energy excluding renewable primary energy resources used as raw materials; RR = use of renewable primary energy resources
used as raw materials; TRR = total use of renewable primary energy resources (EPR + RR); EPNR = use of non-renewable primary energy excluding non-
renewable primary energy resources used as raw materials; RNR = use of non-renewable primary energy resources used as raw materials; TRNR = total use of
non-renewable primary energy resources (EPRN + RNR);
Secondary materials and fuels, and use of water
Modules A1-A3 MS CSR CSNR Net use of fresh water
Unit kg MJ, P.C.I. MJ, P.C.I. m3
Enrocamento 0.00E+00 0.00E+00 0.00E+00 7.67E-03
Tout-Venant 0.00E+00 0.00E+00 0.00E+00 1.15E-02
Pó de Pedra 0.00E+00 0.00E+00 0.00E+00 1.18E-02
Brita 3 0.00E+00 0.00E+00 0.00E+00 1.14E-02
LEGEND:
Product stage
MS = use of secondary material; CSR = use of renewable secondary fuels; CSNR = use of non-renewable secondary fuels.
2.5. Other environmental information describing different waste categories
Modules A1-A3 Hazardous waste disposed Non-hazardous waste disposed Radioactive waste disposed
Unit kg kg kg
Enrocamento 1.49E-04 8.03E+00 1.11E-05
Tout-Venant 1.64E-04 8.03E+00 2.52E-05
Pó de Pedra 1.66E-04 8.03E+00 2.64E-05
Brita 3 1.64E-04 8.03E+00 2.46E-05
LEGENDA:
Product stage
DAPHabitat System 13
2.6. Environmental information describing output flows
Exported energy
Components for Materials for Materials for
re-use recycling energy recovery
Modules A1-A3 Energy carrier 1 … Energy carrier n
Unit kg kg kg MJ MJ MJ
Enrocamento 0.00E+00 8.83E-03 0.00E+00 0.00E+00 0.00E+00 0.00E+00
Tout-Venant 0.00E+00 9.32E-03 0.00E+00 0.00E+00 0.00E+00 0.00E+00
Pó de Pedra 0.00E+00 9.38E-03 0.00E+00 0.00E+00 0.00E+00 0.00E+00
Brita 3 0.00E+00 9.32E-03 0.00E+00 0.00E+00 0.00E+00 0.00E+00
LEGEND:
Product stage
2.7. Information describing the biogenic carbon content at the factory gate
Biogenic carbon content Units Modules A1-A3 (results)
Biogenic carbon content in product Kg C Not Applicable.
Biogenic carbon content in accompanying packaging Kg C Not Applicable.
3. SCENARIOS AND ADDITIONAL TECHNICAL INFORMATION
3.1. Scenario and technical information for module D
Not Applicable.
3.2. Additional information on release of dangerous substances to indoor air, soil, and
water during the use stage
Not Applicable.
14 Sistema DAPHabitat
4. REFERENCES
✓ General Instructions of the DAPHabitat System, Version 2.1, Edition August 2023 (in www.daphabitat.pt);
✓ PCR – basic module for construction products and services. DAPHabitat System. Version 2.3, August 2023 (in
www.daphabitat.pt);
✓ ISO 14025:2009 Environmental declarations and labels – Type III environmental declarations – Principles and
procedures;
✓ EN 15804:2012 + A2:2019 Sustainability of construction works – Environmental product declarations – Core
rules for the product category of construction products;
✓ EN 15942:2021 Sustainability of construction works – Environmental product declarations – Communication
format business-to-business.
✓ SECIL AGREGADOS, “Declaração de Desempenho no 1 - Pó de Pedra,” 2023.
✓ SECIL AGREGADOS, “Declaração de desempenho no 6 - Brita 3,” 2023.
✓ SECIL AGREGADOS, “Declaração de Desempenho no 7 - Tout-Venant de 1a,” 2023.
✓ SECIL AGREGADOS, “Declaração de Desempenho no 8 - Tout-Venant de 2a,” 2023.
✓ SECIL AGREGADOS, “Declaração de Desempenho no 9 - Enrocamento,” 2023.
DAPHabitat System 15
