LOGO OF THE EPD’S OWNER]
DAPH ABITAT S YSTEM E NVIRONMENTAL P RODUCT D ECLARATION
WWW.DAPHABITAT.PT [ACCORDING TO ISO 14025, EN 15804:2012+A2:2019 AND EN 15942]
Declaration number: DAP 008:2024
PLASTERBOARD GYPTEC 13A (STANDARD)
Issue date: 19/09/2024 Valid until: 18/09/2029
GYPTEC IBÉRICA – GESSOS TÉCNICOS, S.A.
Version 1.4. Ed. Março 2024
1
INDEX
1. GENERAL INFORMATION ....................................................................................................... 1
1.1. THE DAPHABITAT SYSTEM .......................................................................................................................... 1
1.2. EPD OWNER ............................................................................................................................................. 1
1.3. INFORMATION CONCERNING THE EPD ............................................................................................................ 3
1.4. DEMONSTRATION OF THE VERIFICATION .......................................................................................................... 3
1.5. EPD REGISTRATION ................................................................................................................................... 3
1.6. PCR (PRODUCT CATEGORY RULES) BASIC MODEL ............................................................................................... 4
1.7. RELEVANT C-PCR (COMPLEMENTARY PRODUCT CATEGORY RULES) ........................................................................ 4
1.8. INFORMATION CONCERNING THE PRODUCT/PRODUCT CLASS ................................................................................ 5
1.9. CALCULATION RULES OF THE LCA ................................................................................................................... 6
1.10. USE OF AVERAGE ENVIRONMENTAL PERFORMANCE ............................................................................................ 7
1.11. TECHNICAL INFORMATION FOR REFERENCE SERVICE LIFE (RSL) ............................................................................. 7
1.12. FLOW DIAGRAM OF INPUT AND OUTPUT OF THE PROCESSES ................................................................................. 8
2. CORE ENVIRONMENTAL IMPACT INDICATORS ........................................................................ 9
2.1. DESCRIPTION OF THE SYSTEM BOUNDARIES ......................................................................................... 9
2.1.1. JUSTIFICATION FOR THE EXEMPTION TO DECLARE MODULES C1, C2, C3, C4 AND D ................................................... 9
2.2. CORE ENVIRONMENTAL IMPACT INDICATORS .................................................................................................. 10
2.3. ADDITIONAL ENVIRONMENTAL IMPACT INDICATORS ......................................................................................... 11
2.4. INDICATORS DESCRIBING RESOURCE USE ........................................................................................................ 12
2.5. OTHER ENVIRONMENTAL INFORMATION DESCRIBING DIFFERENT WASTE CATEGORIES ............................................... 13
2.6. ENVIRONMENTAL INFORMATION DESCRIBING OUTPUT FLOWS ............................................................................ 13
2.7. INFORMATION DESCRIBING THE BIOGENIC CARBON CONTENT AT THE FACTORY GATE ................................................ 14
3. SCENARIOS AND ADDITIONAL TECHNICAL INFORMATION ..................................................... 14
3.1. C1 DE-CONSTRUCTION, DEMOLITION – END OF LIFE OF THE PRODUCT .................................................................. 14
3.2. C2 TRANSPORT – END OF LIFE OF THE PRODUCT .............................................................................................. 14
3.3. C3 WASTE PROCESSING FOR REUSE, RECOVERY AND/OR RECYCLING – END OF LIFE OF THE PRODUCT ........................... 14
3.4. C4 DISPOSAL – END OF LIFE OF THE PRODUCT ................................................................................................. 14
3.5. SCENARIO AND TECHNICAL INFORMATION FOR MODULE D ................................................................................. 15
3.6. ADDITIONAL INFORMATION ON RELEASE OF DANGEROUS SUBSTANCES TO INDOOR AIR, SOIL, AND WATER DURING THE USE
STAGE 15
3.7. OTHER ADDITIONAL INFORMATION .............................................................................................................. 15
4. REFERENCES ........................................................................................................................ 17
SISTEMA DAPHABITAT iii
1. GENERAL INFORMATION
1.1. The DAPHAbitat System
Sustainable Construction Platform
Program operator: www.clusterhabitat.pt
geral@clusterhabitat.pt
Departamento Engenharia Civil
Address: Universidade de Aveiro
3810-193 Aveiro
Email address: deptecnico@clusterhabitat.pt
Telephone number: (+351) 234 401576
www.daphabitat.pt
Website:
Logo
1.2. EPD owner
Name of the owner: Gyptec Ibérica – Gessos Técnicos, S.A.
Rua das Olaias, nº 3
Production site: Parque Industrial e Empresarial da Figueira da Foz
3090-380 Figueira da Foz, Portugal
Telephone: (+351) 233 403 050
E-mail: geral@gyptec.eu
Website: www.gyptec.eu
Logo:
Quality Management System which fulfills the requirements of the following standard ISO
Information concerning the 9001:2015, Registration Number: ES-1595/2009
applicable management
Environmental Management System which fulfills the requirements of the following
Systems:
standard ISO 14001:2015, Registration Number: ES-2017/0224
https://gyptec.eu/en/technical-documentation/
Specific aspects regarding CEA 23620 – production of plaster products for construction
the production:
Conciliate progress and economic growth with an appropriate preservation and protection
of the environment is one of the main business purposes of Gyptec Ibérica – Gessos
Técnicos, S.A. It is therefore concerned to ensure the highest level of satisfaction of all
Organization’s
interested parties, based on a “green economy”, rational and efficient in the use of natural
environmental policy:
resources. https://gyptec.eu/en/quality-and-environment/
To ensure compliance with this purpose, the organization has developed the following
guidelines:
DAPHabitat System 1
1. Comply with customer requirements in order to promote their satisfaction and exceed
their expectations, always respecting and promoting the protection of the Environment and
social responsibility;
2. Comply with applicable laws and regulations on Quality and Environment, as well as
other subscribed compliance obligations, relating to its products and services,
environmental aspects and impacts;
3. Promote continuous improvement of the Integrated Management System by reviewing
the established goals and the adequacy of the organization’s context, of the interested
parties and of the risks and opportunities inherent to its activity, improving the production
process and periodically evaluating its aspects and significant environmental impacts, on a
life-cycle perspective and taking into account future activities to develop;
4. Train, inform and sensitize employees to care about the Environment and Quality in the
tasks they perform, always acting in a conscious, ethical and responsible manner;
5. Prevent pollution by implementing good environmental management practices, with
emphasis on a careful management of waste, favoring reduction, reuse and recycling, and
the preservation of natural resources;
6. Maintain and strengthen its market position through the high quality and innovation of
its products, technical support and compliance with deadlines, thereby addressing the
market competition with confidence, openness and determination to differentiate itself
from the competitors in a positive way;
7. Promote and communicate this Policy with the interested parties as appropriate, with all
employees, as well as with subcontractors, in order to comply with the Quality and
Environment requirements of Gyptec Ibérica – Gessos Técnicos, S.A.
The Administration of Gyptec Ibérica – Gessos Técnicos, S.A. undertakes to periodically
review this Integrated System Policy, which is documented, implemented, maintained and
communicated as appropriate, in order to guarantee its effectiveness.
DAPHabitat System 2
1.3. Information concerning the EPD
Authors: 1) Gyptec Ibérica – Gessos Técnicos, S.A.
- 2) Itecons – Instituto de Investigação e Desenvolvimento Tecnológico para a Construção,
Energia, Ambiente e Sustentabilidade
Contact of the authors: 1) Gyptec Ibérica – Gessos Técnicos, S.A. | Rua das Olaias, nº 3, Parque Industrial e
Empresarial da Figueira da Foz, 3090-380 Figueira da Foz, Portugal
T (+351) 233 403 050 | Dulce Carvalho: geral@gyptec.eu
2) Itecons – Instituto de Investigação e Desenvolvimento Tecnológico para a Construção,
Energia, Ambiente e Sustentabilidade | Rua Pedro Hispano, s/n, 3030-289 Coimbra,
Portugal
T (+351) 239 798 949 | Maria Inês Santos: itecons@itecons.uc.pt
Issue date:
19/09/2024
Registration date:
09/10/2024
Registration number:
DAP 008:2024
Valid until:
18/09/2029
Representativity of the EPD
EPD of one (1) product class, produced in one (1) plant, belonging to a single (1) producer
(location, manufacturer,
(Gyptec Ibérica – Gessos Técnicos, SA).
group of manufacturers):
Where to consult
www.gyptec.eu
explanatory material:
Type of EPD: EPD: cradle-to-gate with modules C1-C4 and module D.
1.4. Demonstration of the verification
External independent verification, accordingly with the standard ISO 14025:2010 and EN 15804:2012+A2:2019
Certification Body Verifier (s)
(CERTIF – Associação para a Certificação) (Ana Cláudia Dias)
1.5. EPD Registration
Programme operator
(Plataforma para a Construção Sustentável)
DAPHabitat System 3
1.6. PCR (product category rules) basic model
Name: PCR: Basic module for construction products and services
Issue date: Edition August 2023
Number of registration on the data RCP-mb001
base:
Version: Version 2.3
Identification and contact of the Marisa Almeida | marisa@ctcv.pt
coordinator (s): Luís Arroja | arroja@ua.pt
José Dinis Silvestre | jose.silvestre@ist.utl.pt
Marisa Almeida | marisa@ctcv.pt
Identification and contact of the
Luís Arroja | arroja@ua.pt
authors:
José Silvestre | jds@civil.ist.utl.pt
Fausto Freire
Cristina Rocha
Ana Paula Duarte
Ana Cláudia Dias
Helena Gervásio
Victor Ferreira
Ricardo Mateus
António Baio Dias
Composition of the Sectorial Panel: -
Consultation period: 18/11/2015 - 18/01/2016
Valid until: 01/06/2027
CEN standard EN 15804 serves as the core Product Category Rules (PCR).
1.7. Relevant c-PCR (Complementary product category rules)
Name: 1. RCP: Wall coverings
2. prEN 17328 :2022 - Complementary product category rules for gypsum-based
construction products
Issue date: 1. June 2022
2. November 2022
Number of registration on the data 1. RCP002:2014
base: 2. -
Version: 1. Version 1.2
2. -
Identification and contact of the 1. Luís Arroja | arroja@ua.pt
coordinator (s):
Marisa Almeida | marisa@ctcv.pt
2. -
Identification and contact of the 1. Marisa Almeida | marisa@ctcv.pt
authors: Luís Arroja | arroja@ua.pt
Ana Cláudia Dias | acdias@ua.pt
2. -
Composition of the Sectorial Panel: 1. RMC - Revestimentos de Mármore Compactos, S.A.; APICER – Associação
Portuguesa da Indústria de Cerâmica; Sonae Indústria, SGPS, S.A.; Gyptec Ibérica
- Gessos Técnicos, S.A.
2. -
Consultation period: 1. 12/08/2013 a 30/11/2013
2. -
Valid until: 1. 01/06/2027
2. -
DAPHabitat System 4
1.8. Information concerning the product/product class
Identification of the product: Plasterboard Gyptec 13A (Standard).
The results presented in this EPD correspond to the most representative
product: Plasterboard Gyptec 13A (Standard). To estimate the environmental
impacts for other thicknesses (Standard Plasterboard 6A, 10A, 15A and 18A) the
results of Plasterboard 13A can be multiplied by the corresponding conversion
factors (see point 3.7. Other additional information).
Illustration of the product:
Brief description of the product: Laminated plasterboard made up of two sheets of paper with high-quality plaster inside.
It is a non-combustible material, resistant to fire and impact, free of harmful substances
and which ensures a healthy indoor environment.
It’s a high energy saving and acoustic performance enhancer, contributing to the comfort
and efficiency of the building.
Main technical characteristics of the
Table 1: Technical characteristics ((https://gyptec.eu/en/technical-documentation/)
product:
Harmonized technical
Essential characteristics Performance
specification
Reaction to Fire A2-s1,d0 EN520
Water Vapor Resistance µ 10 EN 12524
Flexural Strength
Transverse (T) e
Longitudinal (L):
Thickness 6.5mm T: 100.8N; L: 258N
EN520
Thickness 9.5mm T: 160N; L: 400N
Thickness 12.5mm T: 210N; L: 550N
Thickness 15mm T: 250N; L: 650N
Thickness 18mm T: 302.4N; L: 774N
Thermal Conductivity
W/m.ºC (23ºC/ seco)/
W/m.ºC (23ºC/ 50%)
Thickness 6.5mm 0.25 (tabled)
EN 12664
Thickness 9.5mm 0.115/ 0.200
Thickness 12.5mm 0.100/ 0.175
Thickness 15mm 0.105/ 0.185
Thickness 18mm 0.115/ 0.200
Description of the product’s
Typical plasterboard uses are as wall linings, internal partitions or ceilings.
application/use:
Placing on the market / Rules of - EN 520:2004+A1:2009 Gypsum plaster boards. Definitions, requirements and test
application in the market / Technical methods
rules of the product:
- UNE 102043:2013 – “Assembly of constructive systems with laminated plasterboard
(PYL). Partitions, linings and ceilings. Definitions, applications and recommendations.”
- Sistemas Constructivos con Placa de Yeso Laminado, Associación Técnica y Empresarial
del Yeso – A.T.E.D.Y., 4.ª, Edição, January 2011.
- Regulation (EU) no. 305/2011 of the European Parliament and of the Council, of 9
DAPHabitat System 5
March 2011, which establishes harmonized conditions for the marketing of
construction products.
Quality control:
Quality assurance in accordance with the technical standards of the product
Special delivery conditions:
Not applicable
Components and substances to declare:
The gypsum plasterboards are formed by high quality plaster mixed with additives and
encased in two sheets of paper. The products do not contain any substance included in
the Candidate List of Substances of Very High Concern (SVHCs) for authorization with
concentrations higher than 0.1% weight by weight (w/w).
Where explanatory material may be
--
obtained:
History of the LCA studies:
--
1.9. Calculation rules of the LCA
Functional unit: --
Declared unit: 1 m2 of Plasterboard Gyptec 13A (Standard), packaging included.
Parameter Value Unit
Unit of measurement 1 m2
Product weight 5.50E00 kg/m2
Plasterboard Gyptec
Conversion factor to
6A (Standard) 1.82E-01 m2/kg
1 kg
Product weight 6.55E00 kg/m2
Plasterboard Gyptec
Conversion factor to
10A (Standard) 1.53E-01 m2/kg
1 kg
Product weight 7.20E00 kg/m2
Plasterboard Gyptec
Conversion factor to
13A (Standard) 1.39E-01 m2/kg
1 kg
Product weight 9.01E00 kg/m2
Plasterboard Gyptec
Conversion factor to
15A (Standard) 1.11E-01 m2/kg
1 kg
Product weight 12.43E00 kg/m2
Plasterboard Gyptec
Conversion factor to
18A (Standard) 8.05E-02 m2/kg
1 kg
The results presented in this EPD correspond to the most representative product: Plasterboard Gyptec 13A
(Standard). To estimate the environmental impacts for other thicknesses (Standard Plasterboard 6A, 10A, 15A
and 18A) the results of Plasterboard 13A can be multiplied by the corresponding conversion factors (see point
3.7. Other additional information).
System EPD: cradle-to-gate with modules C1-C4 and module D
boundaries:
Figure 1: Life cycle model (cradle-to-gate with modules C1-C4 and module D) of Plasterboard Gyptec (Standard).
Criteria for the According to EN 15804:2012+A2:2019, the cut-off criterion for unit processes is 1% of the total energy consumed
exclusion: and 1% of the total mass of the inputs, with a maximum of 5% of energy usage and mass per module of the life
cycle. The developed LCA includes all available data associated to the product stage [A1-A3] and end of life stage
DAPHabitat System 6
System Boundaries| Cradle-to-gate w ith m odules C and D
A 1 A 2 A 3
Extraction and Productionprocessing ofrawm
aterials
Calcination M ixer Cutting Drying Final Cut Packaging
A 4 A 5
Installation
B1-B7
U se
C1-C4
End-of-life
D
Benefits and loads behind the system
boundary
[C1-C4]. The following processes were not considered:
- Construction of industrial infrastructure and equipment manufacturing;
- Maintenance operations of industrial infrastructure and equipment (in accordance with prEN 17328:2022);
- Burdens of infrastructures associated to transportation of pre-products and raw materials;
- Transport of fuels used at the manufacturing site;
- Consumption and emissions related to human activities such as employee transport, administration
departments and central support services (where this information is not amalgamated into site totals).
Assumption and The year 2020 was considered as the reference year for data collection. This year was selected because it is a
limitations typical year in which total heat produced in the cogeneration from natural gas was used. In the following years,
there were large fluctuations in the prices of natural gas, so over time the amount of heat produced by
cogeneration was reduced.
Quality and other Specific data was used based on the average production of Gyptec Standard Plasterboards in 2020. For processes
characteristics that the producer has no influence over or specific information on, such as the production of raw and auxiliary
about the materials and the production of electricity, generic data from the Ecoinvent v3.10, EF database 2.0 and Agri-
information used footprint 5 databases was used, taking geographical coverage into account.
in the LCA:
The quality of the primary and generic data was assessed based on the levels and criteria of the UN Environment
Global Guidance on LCA database development, taking into account at least 80% of the environmental impacts in
each of the main impact categories. This assessment showed that the quality of the primary data varies between
good and very good and that the quality of the generic data varies between poor (‘occasional situation’) and very
good.
Allocation rules: The industrial unit where Gyptec Standard Plasterboards are manufactured also produces other products (not at
the same time). Considering this, a mass allocation methodology was used to determine which inputs and
outputs are due to manufacturing these products. It should be noted that during the Gypsum Plasterboard
manufacturing no co-products are produced.
Software used for SimaPro v9.6
the assessment:
Background Ecoinvent v3.10
database used for
EF Database v2.0
the LCA:
Agri-footprint 5
Comparability of The EPD of construction products and services cannot be comparable in case they are not produced according to
EPD for EN 15804 and EN 15948 and according to the comparability conditions determined by ISO 14025.
construction
products
1.10. Use of average environmental performance
Not applicable.
1.11. Technical information for Reference Service Life (RSL)
Not applicable. This EPD does not include the use stage (module B).
DAPHabitat System 7
1.12. Flow diagram of input and output of the processes
Electricity
Heat (Natural gas)
Heat (Cogeneration)
Gypsum Calcination Air Emissions
Waste(paper)
Electricity
Water
Mixer Water Emissions
Additives, Paper
Waste
Electricity
Cutting
Waste (rejected products)
Electricity
Heat (Natural gas)
Heat (Cogeneration)
Drying Air Emissions
Waste(rejected products)
Electricity
Final Cut
Waste (rejected products)
Electricity
Packaging materials Packaging
(wood, film, labels, etc.) Waste (rejected products and
packaging materials)
Figure 1: Production process of Standard Gypsum Plasterboard.
The Standard Gypsum Plasterboard production comprises 6 stages: calcination, mixer, cutting, drying, final cut and
packaging. The company Gyptec Ibérica – Gessos Técnicos, S.A. dedicates itself to the production of gypsum
boards. For this purpose, it uses gypsum of two different types, mineral gypsum, which comes from gypsum
mining, and synthetic gypsum, which comes from the desulphurization operations of thermoelectric power
stations. This gypsum is prepared for production, by grinding, drying and calcining, using thermal energy from the
burning of natural gas and mechanical energy from the action of electrically driven mills. At the end of this process,
a hemihydrate powder is obtained, subsequently stored in silos.
In the mixing zone, this hemihydrate powder is mixed with water and additives to form a mass, subsequently
injected between two sheets of paper, to form the plate that is transported to a cutting area, where it is selected
and cut to size for insertion into the dryer.
In the dryer, excess water is removed, using thermal energy from the burning of natural gas, and then the board is
taken to the final cutting and packaging area, where it is subjected to final finishing and packaging.
DAPHabitat System 8
2. CORE ENVIRONMENTAL IMPACT INDICATORS
2.1. DESCRIPTION OF THE SYSTEM BOUNDARIES
(✓= included; ND = module not declared)
BENEFITS AND LOADS
CONSTRUCTION
PRODUCT STAGE USE STAGE END OF LIFE STAGE BEYOND THE SYSTEM
PROCESS STAGE
BOUNDARY
la
y lp p u s la ire wta am R tro p s n a rT g n iru tc a fu n a M tro p s n a rT s s e c o rp n o ita lla ts n i n o itc
u
e s U e c n a n e tn ia M ria p e R tn e m e c a lp e R tn e m h s ib ru fe R e s u y g re n e la n o ita re p O e s u re ta w la n o ita re p O n o itilo m e d ,s n o itc u rts n eo Dc - tro p s n a rT g n is s e c o rp e ts a W la s o p s iD
itn
e to p g n ilc y c e r ,y re v o c e r ,e es u
-
rts R
n
o
C
A1 A2 A3 A4 A5 B1 B2 B3 B4 B5 B6 B7 C1 C2 C3 C4 D
✓ ✓ ✓ ND ND ND ND ND ND ND ND ND ✓ ✓ ✓ ✓ ✓
2.1.1. Justification for the exemption to declare modules C1, C2, C3, C4 and D
Not applicable.
DAPHabitat System 9
2.2. Core environmental impact indicators
The results presented in this EPD correspond to the most representative product: Plasterboard Gyptec 13A
(Standard).
Global warming Depletion
Global
Global warming Global warming potential land use potential of the
warming potential fossil; potential biogenic; and land use stratospheric Acidification
potential total; change; ozone layer; potential; AP
GWP-fossil GWP-biogenic
GWP-total
GWP-luluc ODP
Unit kg CO2 eq. kg CO2 eq. kg CO2 eq. kg CO2 eq. kg CFC 11 eq. mol H+ eq.
Modules A1-A3 2.45E+00 2.53E+00 -8.61E-02 7.68E-03 1.11E-07 5.31E-03
Module C1 0.00E+00 0.00E+00 0.00E+00 0.00E+00 0.00E+00 0.00E+00
Module C2 1.65E-01 1.65E-01 5.35E-05 4.01E-06 3.33E-09 1.84E-04
Module C3 0.00E+00 0.00E+00 0.00E+00 0.00E+00 0.00E+00 0.00E+00
Module C4 8.28E-01 2.26E-01 6.02E-01 9.96E-05 4.62E-09 2.23E-01
Module D 0.00E+00 0.00E+00 0.00E+00 0.00E+00 0.00E+00 0.00E+00
LEGEND:
Product stage
End - of - life stage
Benefits and loads beyond the system boundary
Units expressed by declared unit.
Abiotic Abiotic
Eutrophication Formation depletion depletion
Eutrophication Eutrophication Water (user)
potential potential of potential for potential for
potential potential deprivation
aquatic tropospheric non-fossil fossil
aquatic marine; terrestrial; potential;
freshwater; ozone; resources resources
EP-marine EP-terrestrial WDP
EP-freshwater POCP ADP- potential
minerals&metals ADP-fossil
m3 World eq.
Unit kg P eq. kg N eq. mol N eq. Kg COVNM eq. kg Sb eq. MJ, P.C.I.
deprived
Modules A1-A3 2.39E-04 1.99E-03 1.43E-02 6.80E-03 1.21E-05 3.83E+01 1.42E+00
Module C1 0.00E+00 0.00E+00 0.00E+00 0.00E+00 0.00E+00 0.00E+00 0.00E+00
Module C2 1.18E-06 3.85E-05 4.25E-04 4.01E-04 5.40E-09 2.16E+00 9.17E-04
Module C3 0.00E+00 0.00E+00 0.00E+00 0.00E+00 0.00E+00 0.00E+00 0.00E+00
Module C4 2.87E-05 1.27E-03 4.90E-03 1.52E-02 5.10E-08 3.61E+00 -7.82E-01
Module D 0.00E+00 0.00E+00 0.00E+00 0.00E+00 0.00E+00 0.00E+00 0.00E+00
LEGENDA: “The results obtained for the indicators “Abiotic depletion potential for non-
fossil resources (ADP-minerals&metals)”, “Abiotic depletion potential for fossil
Product stage
resources potential (ADP-fossil)” and “Water (user) deprivation potential (WDP)”
End - of - life stage should be used with caution since the uncertainties associated with them are
high or there is little experience with the indicator.”
Benefits and loads beyond the system boundary
Units expressed by declared unit.
DAPHabitat System 10
2.3. Additional environmental impact indicators
Potential Potential
Potential Potential Potential
incidence of Human Comparative
Comparative Comparative Toxic Potential soil
disease due exposure Toxic Unit for
Toxic Unit for Unit for humans, quality index
to PM efficiency humans, not
ecosystems cancer effects
emissions relative to U235 cancer effects SQP
IRP ETP-fw HTP-c
PM HTP-nc
Disease
Unit kBq U 235 eq. CTUe CTUh CTUh -
incidence
Modules A1-A3 ND ND ND ND ND ND
Module C1 ND ND ND ND ND ND
Module C2 ND ND ND ND ND ND
Module C3 ND ND ND ND ND ND
Module C4 ND ND ND ND ND ND
Module D ND ND ND ND ND ND
LEGEND:
Product stage
End-of-life stage
Benefits and loads beyond the system boundary
NOTES:
Values expressed by declared unit. “ND” means Not Declared.
The impact indicator “POTENTIAL HUMAN EXPOSURE EFFICIENCY RELATIVE TO U235” focuses mainly on the possible impact of a low dose of ionising
radiation on human health resulting from the nuclear fuel cycle. It does not consider effects arising from possible nuclear accidents, occupational
exposure or the disposal of radioactive waste in underground facilities. Potential ionising radiation from soil, radon and some building materials is also
not measured by this indicator.
The results of the indicators “POTENTIAL COMPARATIVE TOXIC UNIT FOR ECOSYSTEMS (ETP-FW)”, “POTENTIAL COMPARATIVE TOXIC UNIT FOR
HUMANS, CANCER EFFECTS”, “POTENTIAL COMPARATIVE TOXIC UNIT FOR HUMANS, NOT CANCER EFFECTS” and “POTENTIAL SOIL QUALITY INDEX”
should be used with caution as the uncertainties associated with them are high or there is little experience with the indicator.
DAPHabitat System 11
2.4. Indicators describing resource use
The results presented in this EPD correspond to the most representative product: Plasterboard Gyptec 13A
(Standard).
Primary energy
EPR RR TRR EPNR RNR TRNR
Unit MJ, P.C.I. MJ, P.C.I. MJ, P.C.I. MJ, P.C.I. MJ, P.C.I. MJ, P.C.I.
Modules A1-A3 2.00E+00 8.90E-01 2.89E+00 3.81E+01 1.58E-01 3.83E+01
Module C1 0.00E+00 0.00E+00 0.00E+00 0.00E+00 0.00E+00 0.00E+00
Module C2 7.49E-03 0.00E+00 7.49E-03 2.16E+00 0.00E+00 2.16E+00
Module C3 0.00E+00 0.00E+00 0.00E+00 0.00E+00 0.00E+00 0.00E+00
Module C4 1.22E-01 0.00E+00 1.22E-01 3.61E+00 0.00E+00 3.61E+00
Module D 0.00E+00 0.00E+00 0.00E+00 0.00E+00 0.00E+00 0.00E+00
EPR = use of renewable primary energy excluding renewable primary
LEGEND: energy resources used as raw materials; RR = use of renewable primary
energy resources used as raw materials; TRR = total use of renewable
Product stage
primary energy resources (EPR + RR); EPNR = use of non-renewable primary
End-of-life stage energy excluding non-renewable primary energy resources used as raw
materials; RNR = use of non-renewable primary energy resources used as
Benefits and loads beyond the system boundary raw materials; TRNR = total use of non-renewable primary energy resources
Units expressed by declared unit. (EPRN + RNR);
Secondary materials and fuels, and use of water
MS CSR CSNR Net use of fresh water
Unit kg MJ, P.C.I. MJ, P.C.I. m3
Modules A1-A3 3.48E-01 0.00E+00 0.00E+00 1.29E-01
Module C1 0.00E+00 0.00E+00 0.00E+00 0.00E+00
Module C2 0.00E+00 0.00E+00 0.00E+00 5.52E-05
Module C3 0.00E+00 0.00E+00 0.00E+00 0.00E+00
Module C4 0.00E+00 0.00E+00 0.00E+00 -1.77E-02
Module D 0.00E+00 0.00E+00 0.00E+00 0.00E+00
LEGEND:
Product stage MS = use of secondary material; CSR = use of renewable secondary fuels;
CSNR = use of non-renewable secondary fuels.
End-of-life stage
Benefits and loads beyond the system boundary
Units expressed by declared unit.
DAPHabitat System 12
2.5. Other environmental information describing different waste categories
The results presented in this EPD correspond to the most representative product: Plasterboard Gyptec 13A
(Standard).
Hazardous waste disposed Non-hazardous waste disposed Radioactive waste disposed
Unit kg kg kg
Modules A1-A3 1.80E-04 3.55E-02 2.31E-05
Module C1 0.00E+00 0.00E+00 0.00E+00
Module C2 1.43E-05 6.58E-05 2.03E-07
Module C3 0.00E+00 0.00E+00 0.00E+00
Module C4 2.99E-05 7.31E+00 3.40E-06
Module D 0.00E+00 0.00E+00 0.00E+00
LEGENDA:
Product stage
End-of-life stage
Benefits and loads beyond the system boundary
Units expressed by declared unit.
2.6. Environmental information describing output flows
The results presented in this EPD correspond to the most representative product: Plasterboard Gyptec 13A
(Standard).
Components for re- Materials for Materials for energy
Exported energy
use recycling recovery
Unit kg kg kg MJ
Modules A1-A3 0.00E+00 1.95E-02 0.00E+00 0.00E+00
Module C1 0.00E+00 0.00E+00 0.00E+00 0.00E+00
Module C2 0.00E+00 0.00E+00 0.00E+00 0.00E+00
Module C3 0.00E+00 0.00E+00 0.00E+00 0.00E+00
Module C4 0.00E+00 0.00E+00 0.00E+00 0.00E+00
Module D 0.00E+00 0.00E+00 0.00E+00 0.00E+00
LEGEND:
Product stage
End-of-life stage
Benefits and loads beyond the system boundary
Units expressed by declared unit.
DAPHabitat System 13
2.7. Information describing the biogenic carbon content at the factory gate
The results presented in this EPD correspond to the most representative product: Plasterboard Gyptec 13A
(Standard).
Biogenic carbon content* Units** Modules A1-A3 (results)
Biogenic carbon content in product kg C 1.76E-01
Biogenic carbon content in accompanying packaging kg C 2.93E-02
* 1 kg biogenic carbon is equivalent to 44/12 kg of CO2.
** This information can be omitted whenever the content of biogenic carbon in the product, or in the respective packaging, is less than 5% of the
mass of the product, or the respective packaging.
3. SCENARIOS AND ADDITIONAL TECHNICAL INFORMATION1
3.1. C1 De-construction, demolition – End of life of the product
According to prEN 17328:2022, “The deconstruction and/or dismantling (C1) of gypsum-based products often
occurs as part of the demolition of the entire building. Due to regulatory requirements, gypsum wastes need to be
separated from other mineral deconstruction waste. That is why selective dismantling needs to be applied, either
entirely manually or with some electrical devices. Therefore, the environmental impact of deconstructing gypsum-
based products is assumed to be very small compared to the deconstruction of other (mineral) building products
and therefore, the corresponding environmental impacts can be neglected on the grounds of materiality”. The
deconstruction of Gyptec Standard Plasterboard is typically carried out manually, without associated consumption,
so the impacts are zero.
3.2. C2 Transport – End of life of the product
In the transport of the gypsum plasterboard waste, it was considered that the waste operators are within a radius
of 50 km, according to primary information from the manufacturer. It was also assumed that the waste was
transported by lorry with a gross weight of 3.5-7.5 tonnes.
3.3. C3 Waste processing for reuse, recovery and/or recycling – End of life of the product
It was considered that, in the present moment, no waste is sent to reuse, recycling or energy recovery. The impact
is considered zero.
3.4. C4 Disposal – End of life of the product
A scenario of landfill disposal (100%) was considered. The landfill scenario was defined based on a conservative
approach and primary information from the manufacturer (current situation).
1 IF THERE IS NO ADDITIONAL TECHNICAL INFORMATION AND NO SCENARIOS HAVE BEEN CARRIED OUT, ENTRIES SHOULD BE FILLED IN WITH "NOT APPLICABLE”.
DAPHabitat System 14
3.5. Scenario and technical information for module D
At present there are no processes for re-use or recovery. Therefore, the potential benefits beyond the system
boundaries (D) are zero.
3.6. Additional information on release of dangerous substances to indoor air, soil, and
water during the use stage
Gyptec gypsum boards are rated A+ for indoor air quality. This qualification comes from the French
regulations for emissions of volatile pollutants, with Category A+ being the best indoor air quality
classification, meaning very low or no emissions of substances in indoor air, such as VOCs (volatile organic
compound). https://gyptec.eu/en/gyptec-the-most-advantageous-gypsum-board/
3.7. Other additional information
ADDITIONAL CERTIFICATES:
• AENOR Product Certificate [N] according to RP035.09 Private Regulation of the AENOR brand for
Gyptec plasterboards;
• Certificate Sustainable Value for Gyptec plasterboards according to ISO 14024.
FACTORS TO ESTIMATE ENVIRONMENTAL IMPACTS FOR OTHER THICKNESSES:
Standard plasterboards are produced in different format. To estimate environmental impacts for other
thicknesses, results might be multiplied by the corresponding factor in the following table.
Conversion factors
Plasterboard 6A Plasterboard 10A Plasterboard 13A Plasterboard 15A Plasterboard 18A
GWP-Total
1.00 0.93 1.00 1.19 1.52
(kg CO eq.)
2
GWP-Fossil
0.97 0.91 1.00 1.22 1.62
(kg CO eq.)
2
GWP-Biogenic
1.16 1.01 1.00 1.01 0.92
(kg CO eq.)
2
GWP-Luluc
1.03 0.93 1.00 1.08 1.14
(kg CO eq.)
2
ODP
279.94 0.91 1.00 1.23 1.67
(kg CFC-11 eq.)
AP
0.76 0.91 1.00 1.26 1.75
(mol H+ eq.)
EP-Freshwater
1.38 0.91 1.00 1.08 1.17
(kg P eq.)
EP-Marine
1.09 0.93 1.00 1.15 1.38
(kg N eq.)
EP-Terrestrial
1.19 0.92 1.00 1.18 1.46
(mol N eq.)
POCP
0.85 0.90 1.00 1.24 1.68
(kg NMVOC eq.)
ADP-Minerals&metals
1.19 1.03 1.00 1.09 1.12
(kg Sb eq.)
ADP-Fossil
0.93 0.91 1.00 1.22 1.62
(MJ)
WDP
1.05 0.92 1.00 1.14 1.36
(m3 world eq. deprived)
DAPHabitat System 15
END OF LIFE:
A scenario of landfill disposal (100%) was considered. The landfill scenario was defined based on a conservative
approach and primary information from the manufacturer (current situation). However, Gyptec plasterboard can
be recycled in a closed loop into new product without any loss in quality or performance. Gyptec
plasterboard waste from deconstruction should consigned to a recycling center.
DAPHabitat System 16
4. REFERENCES
✓ EN 15804:2012+A2:2019 Sustainability of construction works – Environmental product declarations – Core
rules for the product category of construction products;
✓ International Organization for Standardization (ISO). EN ISO 14040:2006. Environmental management – life
cycle assessment –principles and framework, 2006.
✓ International Organization for Standardization (ISO). EN ISO 14044:2006. Environmental management ‒ Life
cycle assessment ‒ Requirements and guidelines, 2006.
✓ International Organization for Standardization (ISO). ISO 14025:2006. Environmental labels and declarations —
Type III environmental declarations — Principles and procedures, 2006.
✓ European Standard. EN 15804:2012+A2:2019. Sustainability of construction works - Environmental product
declarations - Core rules for the product category of construction products, 2019.
✓ European Standard. CEN/TR 15941:2010. Sustainability of construction works - Environmental product
declarations - Methodology for selection and use of generic data, 2010.
✓ EN 15942:2021 Sustainability of construction works – Environmental product declarations – Communication
format business-to-business.
✓ European Standard. prEN 17328:2022. Complementary product category rules for gypsum-based construction
products, 2022.
✓ General Instructions for the Daphabitat System, Version 2.1. Aveiro, August 2023.
✓ PCR Basic module for construction products and services, version 2.3. Aveiro, August 2023.
✓ PCR Wall covering, version 1.2, Aveiro, June 2022.
✓ SimaPro software, PRé Consultants bv 1990-2024, Release 9.6.0.1.
✓ FitzGerald D., Bourgault G., Vadenbo C., Sonderegger T., Symeonidis A., Fazio S., Mutel C., Müller J., Dellenbach
D., Stoikou N., Baumann D., Clementi M., Ioannou I., Cirone F., Superti V., Beckert P., Treichel A., Kaarlela O.,
Kunde S., Valsasina L., Moreno Ruiz E. Documentation of changes implemented in the ecoinvent database
v3.10. Ecoinvent Association, Zürich, Switzerland, 2023.
✓ European Commission. Environmental Footprint (EF) database 2.0, Version 1.1, 2020.
✓ Blonk Agri-footprint BV. (2019). Agri-Footprint – Part 2 – Description of data. Gouda, the Netherlands.
✓ PRé, SimaPro Database Manual Methods Library, 2024.
DAPHabitat System 17
