LOGO OF THE EPD’S OWNER]
DAPH ABITAT S YSTEM E NVIRONMENTAL P RODUCT D ECLARATION
WWW.DAPHABITAT.PT [ACCORDING TO ISO 14025, EN 15804:2012+A2:2019 AND EN 15942]
Declaration number: DAP 012:2024
COLD-FORMED WELDED STRUCTURAL HOLLOW SECTIONS OF
NON-ALLOY AND FINE GRAINS STEELS
ISSUE DATE: 28/10/2024 VALID UNTIL: 27/10/2029
FERPINTA - Indústrias de tubos de Aço de Fernando Pinho Teixeira, S.A.
Version 1.4.1 Ed. March 2024
1
INDEX
1. GENERAL INFORMATION ...................................................................................................................... 2
1.1. The DAPHAbitat System ................................................................................................................................... 2
1.2. EPD owner ........................................................................................................................................................ 2
1.3. Information concerning the EPD ....................................................................................................................... 3
1.4. Demonstration of the verification .................................................................................................................... 3
1.5. EPD Registration ............................................................................................................................................... 3
1.6. PCR (product category rules) basic model ........................................................................................................ 4
1.7. Relevant c-PCR (Complementary product category rules) ................................................................................ 4
1.8. Information concerning the product/product class .......................................................................................... 5
1.9. Calculation rules of the LCA .............................................................................................................................. 6
1.10. Use of average environmental performance .................................................................................................... 7
1.11. Technical information for Reference Service Life (RSL) ..................................................................................... 7
1.12. Flow diagram of input and output of the processes.......................................................................................... 8
2. CORE ENVIRONMENTAL IMPACT INDICATORS ...................................................................................... 9
2.1. Description of the system boundaries .............................................................................................................. 9
2.1.1. Justification for the exemption to declare modules C1, C2, C3, C4 and D .................................................... 9
2.2. Core environmental impact indicators ........................................................................................................... 10
2.3. Additional environmental impact indicators .................................................................................................. 11
2.4. Indicators describing resource use ................................................................................................................. 12
2.5. Other environmental information describing different waste categories ....................................................... 13
2.6. Environmental information describing output flows ...................................................................................... 13
2.7. Information describing the biogenic carbon content at the factory gate ........................................................ 14
3. SCENARIOS AND ADDITIONAL TECHNICAL INFORMATION ................................................................... 14
3.1. C2 Transport – End-of-life of the product ....................................................................................................... 14
3.2. C3 Waste processing for reuse. recovery and/or recycling – End-of-life of the product .................................. 14
3.3. C4 Disposal – End-of-life of the product ......................................................................................................... 14
3.4. Scenario and technical information for module D .......................................................................................... 14
3.5. Additional information on release of dangerous substances to indoor air, soil, and water during the use stage
15
4. REFERENCES ...................................................................................................................................... 15
DAPHabitat System 1
1. GENERAL INFORMATION
1.1. The DAPHAbitat System
Sustainable Construction Platform
Program operator: www.clusterhabitat.pt
geral@clusterhabitat.pt
Departamento Engenharia Civil
Address: Universidade de Aveiro
3810-193 Aveiro
Email address: deptecnico@clusterhabitat.pt
Telephone number: (+351) 234 401576
Website: www.daphabitat.pt
Logo
1.2. EPD owner
Name of the owner:
FERPINTA – Indústrias de Tubos de Aço de Fernando Pinho Teixeira, S.A.
Rua 13 de Julho, nº295
Production site:
3720-011 Carregosa, Oliveira de Azeméis
Rua 13 de Julho, nº295
Address (head office):
3720-011 Carregosa, Oliveira de Azeméis
Telephone: +351 256 411 420
info@ferpinta.pt
E-mail:
ana.amorim.fer@ferpinta.pt
Website: www.ferpinta.pt
Logo:
Information concerning the
NP EN ISO 9001:2015 – Quality Management Systems
applicable management
NP EN ISO 14001:2015 – Environmental Management System
Systems: NP EN ISO 50001:2019 – Energy Management Systems
Specific aspects regarding
Main CAE: 24200 – Manufacture of tubes, pipes, hollow profiles and related fittings, of steel
the production:
FERPINTA aims to build a better future by producing pipes, profiles, shapes, and bands of steel that we
Organization’s want to get further and further. Aware of its mission, FERPINTA seeks to adopt methods and
technologies that prevent pollution protect the environment, using natural resources in an effective
environmental policy:
way, and ensuring that FERPINTA products are developed considering the life cycle perspective. The
full Management Policy can be consulted at: www.grupoferpinta.com/imagem/PolíticaGestão_FPT.pdf.
DAPHabitat System 2
1.3. Information concerning the EPD
Authors:
Ana Cláudia Dias
Contact of the authors: Address: University of Aveiro, Campus Universitário de Santiago, 3810-193 Aveiro, Portugal
Phone number: +351 234 370 200
E-mail: acdias@ua.pt
Issue date:
28/10/2024
Registration date:
18/11/2024
Registration number:
DAP 012:2024
Valid until:
01/05/2028
Representativity of the EPD
(location, manufacturer,
EPD of one (1) product category, produced in one (1) industrial plant from one (1) producer
group of manufacturers):
Where to consult
www.ferpinta.pt
explanatory material:
Type of EPD: Cradle-to-gate EDP (A1-A3) with modules C and D
1.4. Demonstration of the verification
External independent verification, accordingly with the standard ISO 14025:2010 and EN 15804:2012+A2:2019
Certification Body Verifier
(CERTIF – Associação para a Certificação) (Marisa Almeida)
1.5. EPD Registration
Programme operator
(Plataforma para a Construção Sustentável)
DAPHabitat System 3
1.6. PCR (product category rules) basic model
Name: PCR: Basic module for construction products and services
Issue date: Edition August 2023
Number of registration on the data
RCP-mb001
base:
Version: Version 2.3
Marisa Almeida | marisa@ctcv.pt
Identification and contact of the
Luís Arroja | arroja@ua.pt
coordinator (s):
José Dinis Silvestre | jose.silvestre@ist.utl.pt
Marisa Almeida | marisa@ctcv.pt
Identification and contact of the
Luís Arroja | arroja@ua.pt
authors:
José Silvestre | jds@civil.ist.utl.pt
Fausto Freire
Cristina Rocha
Ana Paula Duarte
Ana Cláudia Dias
Helena Gervásio
Victor Ferreira
Ricardo Mateus
António Baio Dias
Composition of the Sectorial Panel: -
Consultation period: 18/11/2015 - 18/01/2016
Valid until: 01/06/2027
CEN standard EN 15804 serves as the core Product Category Rules (PCR)
1.7. Relevant c-PCR (Complementary product category rules)
Not applicable.
DAPHabitat System 4
1.8. Information concerning the product/product class
Identification of the product: Cold-formed welded structural hollow sections of non-alloy and fine steel grains steels
Illustration of the product:
Brief description of the product: FERPINTA’s range of structural hollow sections consists of round, square, and rectangular
products, longitudinally welded, cold-formed, and without subsequent heat treatment.
Structural hollow sections are produced according to the EN 10219-1 standard, with a
diameter range of 16 to 323.9 mm, and with a wall thickness of 1.5 to 12.5 mm. The tube can
be supplied in black (rough rolled) or pickled. The entire range of cold-formed welded
structural hollow sections produced at FERPINTA is included in the EPD.
Main technical characteristics of the The technical properties of the cold-formed welded structural hollow sections comply with the
product: requirements of the EN 10219-1:2006 and EN 10219-2:2006 standards, as indicated in Table 1.
The mechanical properties are presented in Table 2.
Table 1: General properties
Properties Standard Section
Tolerances on dimension and shape EN 10219-2 6
Elongation EN 10219-1 6.7.1, Tables A.3, B.4 and B.5
Tensile strength and yield strength EN 10219-1 6.7.1, Tables A.3, B.4 and B.5
Impact strength EN 10219-1 6.7.2, Tables A.3, B.4 and B.5
Weldability EN 10219-1 6.6, Tables A.1, B.1, B.2 and 6.8.1
Durability EN 10219-1 6.8.2
Table 2: Mechanical properties, according to the EN 10219-1:2006 standard
Mechanical properties
Minimum
Minimum Minimum impact energy, KV
yield Tensile strength, Rm
elongation, A (J)
Steel grade strength, (MPa)
(%)
ReH (MPa)
Thickness (mm) At test temperature of
≤ 16mm < 3 ≥ 3 ≤ 40 ≤ 40 -50 ◦C -20 ◦C 0 ◦C 20 ◦C
S235JRH 235 360-510 360-510 24 - - - 27
S275J0H 275 430-580 410-560 20 - - 27 -
S275J2H 275 430-580 410-560 20 - 27 - -
S355J0H 355 510-680 470-630 20 - - 27 -
S355J2H 355 510-680 470-630 20 - 27 - -
S355K2H 355 510-680 470-630 20 - 40 - -
S420MH 420 - 500-660 19 - 40 - -
S420MLH 420 - 500-660 19 27 - - -
S460MH 460 - 530-720 17 - 40 - -
S460MLH 460 - 530-720 17 27 - - -
S460NH 460 - 540-720 17 - 40 - -
S460NLH 460 - 540-720 17 27 - - -
Note: specific information in the technical sheet of the product and/or on the label.
Description of the product’s • For use in metallic structures or mixed structures - metal and concrete.
application/use:
Placing on the market / Rules of • EN 10219;
application in the market / Technical • Certificate of conformity of the factory production control, according to Regulation
rules of the product: 305/2011/EU.
DAPHabitat System 5
Quality control: According to EN 10219-1, Section 7.3, Table 2 – Inspection programme for hollow sections of
non-alloy steels (specific inspection).
Special delivery conditions: Not applicable.
Components and substances to The product does not contain substances from the candidate list of substances of very high
declare: concern for authorisation when their content exceeds the limits for registration with the
European Chemicals Agency (concentration higher than 0.1% in mass).
Where explanatory material may be
www.ferpinta.pt
obtained:
History of the LCA studies: -
1.9. Calculation rules of the LCA
Functional unit: Not applicable.
Declared unit: 1 tonne (t) of cold-formed welded structural hollow sections, with a density of 7,850 kg/m3,
ready for delivery.
System boundaries: The assessed system includes modules A1-A3 (product stage), C (end-of-life stage), and D
(benefits and loads beyond the system boundary). In the end-of-life stage, the impacts of
module C1 (deconstructions and demolition) were excluded due to the lack of information.
A more detailed description of the system boundary is presented in Section 2.1.
The LCA considered all the production processes of the materials and energy consumed in
Criteria for the exclusion:
the system, as well as the management processes of the wastes generated, for which
inventory data were available. It should be noted that the flows of materials excluded in the
structural hollow sections production process are equal to 0.02% of the total mass of inputs
to that process and, therefore, are covered by the cut-off criteria defined in the ‘PCR – Basic
Model’ document. More specifically, their mass contributes less than 1% to the total mass
of the inputs and less than 5% to the total mass of inputs to each information module.
The consumption of energy and water in the administrative areas, as well as the production
of wastewater and wastes from these areas, were excluded. The environmental burdens
from the construction and maintenance of infrastructures and equipment (capital goods)
were also excluded, except those associated with the maintenance of machinery and
equipment used in the production of structural hollow sections.
Assumption and limitations The results of the environmental impacts and remaining indicators shown in this EDP refer
to the year 2023 and constitute average values for the entire range of cold-formed welded
structural hollow sections produced by FERPINTA.
For the production process of cold-formed welded structural hollow sections, real and
Quality and other characteristics
specific data from the production plant have been used. The only exception is emissions to
about the information used in the
air resulting from the burning of diesel consumed in internal transport operations, which
LCA:
have been calculated based on emission factors due to the lack of measured values.
For steel production, real data from one supplier and generic data from the Ecoinvent
database have been used. This database was also used for the remaining processes, meeting
the quality criteria defined for generic data (time-related, geographical and technological
representativeness, plausibility, completeness, consistency, etc.). Whenever possible, the
original processes from Ecoinvent were adapted to better represent reality, for example by
changing the mix of energy sources of electricity consumed considering the country where
processes take place.
According to the criteria defined in Table E.1 of Annex E of the EN 15804 standard, defined
by “UN Environment Global Guidance on LCA database development”, the majority of
relevant data have very good quality, although some data have good quality. The quality of
the data used in module D is also very good, except for the geographical representativeness
of some processes, which is considered good.
In addition to cold-formed welded structural hollow sections, FERPINTA also produces other
Allocation rules:
types of tubes, which constitutes a multifunctionality situation. To determine the inputs and
outputs associated only with the production of cold-formed welded structural hollow
sections, the unit process subdivision procedure was first adopted. Therefore, only
operations associated with the production of the product under assessment were
considered and the operations associated with the remaining products were excluded.
Then, for the included operations, an allocation procedure based on the mass of the
different products produced was applied.
Software used for the assessment: SimaPro version 9.5.0.2.
DAPHabitat System 6
Background database used for the Ecoinvent version 3.9.1 database published in December 2022; “cut-off” approach.
LCA:
Comparability of EPD for construction The EPD of construction products and services cannot be comparable in case they are not
products produced according to EN 15804 and EN 15948 and according to the comparability
conditions determined by ISO 14025.
1.10. Use of average environmental performance
This EPD presents the average environmental performance of the entire range of cold-formed welded structural
hollow sections produced by FERPINTA in 2023. The variability of the environmental performance between specific
products is not relevant.
1.11. Technical information for Reference Service Life (RSL)
Not applicable.
DAPHabitat System 7
1.12. Flow diagram of input and output of the processes
A1 -extraction and processing of raw materials
A2 - transport
A3 -manufacturing
Reception of raw material
Longitudinal cut
s
e
c n
re
w Materials for
a o
n e tn
ia
Tube production g n ilot recycling
M o
C
Storage
Despatch
Cold-formed welded structural
hollow sections
C -end of life
C2: transport Materials for
C3: waste processing recycling
C4: waste disposal
D -benefits and loads beyond the system boundary
Recycling of structural hollow sections at the end of life
Recycling of steel scrap from the manufacturing process
System boundaries
Figure 1: Life cycle stages and unit processes.
DAPHabitat System 8
2. CORE ENVIRONMENTAL IMPACT INDICATORS
2.1. Description of the system boundaries
(✓= included; ND = module not declared)
BENEFITS AND LOADS
CONSTRUCTION
PRODUCT STAGE USE STAGE END-OF-LIFE STAGE BEYOND THE SYSTEM
PROCESS STAGE
BOUNDARY
la
y lp p u s la ire ta m w a R tro p s n a rT g n iru tc a fu n a M tro p s n a rT s s e c o rp n o ita lla ts n i n o itc u
rts
e s U e c n a n e tn ia M ria p e R tn e m e c a lp e R tn e m h s ib ru fe R e s u y g re n e la n o ita re p O e s u re ta w la n o ita re p O n o itilo m e d ,s n o itc u rts n eo Dc - tro p s n a rT g n is s e c o rp e ts a W la s o p s iD
itn
e to p g n ilc y c e r ,y re v o c e r ,e
s
u
n o
C
e R-
A1 A2 A3 A4 A5 B1 B2 B3 B4 B5 B6 B7 C1 C2 C3 C4 D
✓ ✓ ✓ ND ND ND ND ND ND ND ND ND ND ✓ ✓ ✓ ✓
The product stage (module A1-A3) considers the manufacturing of structural hollow sections, as well as the extraction,
processing, and transport of raw material (hot rolled steel coils), ancillary materials, packaging materials, and energy vectors,
and also waste processing until the end-of-waste state is reached or until the end-of-life.
The manufacturing process of structural hollow sections starts with raw material reception (steel coils) where the properties of
the material are confirmed. The next operation is longitudinal cutting where steel coils are cut in strips with width compatible
with the diameters/dimensions of the hollow sections to be produced. After this operation, the material enters in the tube
production/conformation line.
The strip resulting from the longitudinal cutting operation are unrolled and sent to conformation (when a slit is unrolled, the
slits are connected by butt joint welding). In the hollow section conformation is used a set of rollers that gives the strip the
configuration near of a circle, lightly open on the edge. The next operation is the longitudinal electric resistance welding, where
the outer excesses of the weld are eliminated by rectification. The tube, continuously moving, is cooled and calibrated to
achieve the intended cross-section – circular, rectangular or square, according to the normative requirements. Before cutting in
the intended length, a protective oil may be applied for protection against corrosion. The next operations are storage and
expedition.
In the end-of-life stage, the impacts from module C1 (deconstruction and demolition) were excluded because, although
mechanized deconstruction and demolition of structures built with the structural hollow sections may occur, there is no
information available for the quantification of the respective impacts. The following modules were considered:
• C2 – transport of the structural hollow sections from the place of deconstruction or demolition until the end-of-life
(recycling);
• C3 – includes the activities taking place before recycling, in particular, sorting and pressing of the hollow sections;
• C4 – corresponds to waste final disposal; the environmental impacts are null as the hollow sections are recycled.
Module D considers the environmental benefits and loads associated with recycling the structural hollow sections at the end-
of-life and of the steel scrap generated in the hollow sections manufacturing process, assuming that steel recycling will avoid
the production of steel from primary material.
2.1.1. Justification for the exemption to declare modules C1, C2, C3, C4 and D
Not applicable.
DAPHabitat System 9
2.2. Core environmental impact indicators
Depletion
Global Global warming
Global warming Global warming potential of the
warming potential fossil; potential biogenic; potential land use stratospheric Acidification
potential total; and land use change; ozone layer; potential; AP
GWP-fossil GWP-biogenic
GWP-total GWP-luluc
ODP
Unit kg CO2 eq. kg CO2 eq. kg CO2 eq. kg CO2 eq. kg CFC 11 eq. mol H+ eq.
Module A1-A3 1.81E+03 1.80E+03 1.42E+01 1.10E+00 3.42E-05 9.93E+00
Module C2 2.44E+01 2.44E+01 1.34E-02 4.65E-04 5.04E-07 5.99E-02
Module C3 1.26E+01 1.24E+01 1.66E-01 2.04E-02 2.09E-07 1.02E-01
Module C4 0.00E+00 0.00E+00 0.00E+00 0.00E+00 0.00E+00 0.00E+00
Module D -8.70E+02 -8.60E+02 -1.12E+01 2.90E-01 -1.70E-05 -3.40E+00
LEGEND:
Product stage
End-of-life stage
Benefits and loads beyond the system boundary
Values expressed per declared unit (1 t of cold-formed welded structural hollow sections).
Eutrophication Abiotic Abiotic
Eutrophication Formation
p ao qt uen att ii ca l potential Eu ptr oo tp eh nic ta iati lo n potential of pod te ep nle tit aio l fn o r pod te ep nle tit aio l fn o r W dea pte rir v ( au ts ioe nr)
freshwater; aquatic terrestrial; tropospheric non-fossil fossil potential;
marine; ozone; resources resources
EP- EP-terrestrial potential WDP
EP-marine POCP ADP-
freshwater minerals&metals ADP-fossil
m3 World eq.
Units kg P eq. kg N eq. mol N eq. Kg COVNM eq. kg Sb eq. MJ. P.C.I
deprived
Module A1-A3 1.09E-01 2.05E+00 2.23E+01 9.79E+00 6.11E-03 2.00E+04 1.05E+02
Module C2 1.90E-05 2.33E-02 2.45E-01 9.67E-02 8.15E-07 3.12E+02 2.89E-01
Module C3 1.16E-04 4.41E-02 4.80E-01 1.42E-01 5.36E-07 1.93E+02 1.33E+00
Module C4 0.00E+00 0.00E+00 0.00E+00 0.00E+00 0.00E+00 0.00E+00 0.00E+00
Module D -4.07E-02 -6.87E-01 -7.96E+00 -4.24E+00 -7.66E-03 -7.51E+03 -8.03E+01
LEGENDA:
Product stage
End-of-life stage
Benefits and loads beyond the system boundary
Values expressed per declared unit (1 t of cold-formed welded structural hollow sections).
The results obtained for the indicators “Abiotic depletion potential for non-fossil resources (ADP-minerals&metals)”, “Abiotic depletion potential for fossil
resources potential (ADP-fossil)” and “Water (user) deprivation potential (WDP)” should be used with caution since the uncertainties associated with them are
high or there is little experience with the indicator.
DAPHabitat System 10
2.3. Additional environmental impact indicators
Potential Potential Potential Potential Potential
incidence of Human Comparative
Comparative Comparative Toxic Potential soil
disease due exposure Toxic Unit for
Toxic Unit for Unit for humans. quality index
to PM efficiency humans. not
ecosystems cancer effects
emissions relative to U235 cancer effects SQP
PM IRP ETP-fw HTP-c HTP-nc
Disease
Unit kBq U 235 eq. CTUe CTUh CTUh -
incidence
Module A1-A3 ND ND ND ND ND ND
Module C2 ND ND ND ND ND ND
Module C3 ND ND ND ND ND ND
Module C4 ND ND ND ND ND ND
Module D ND ND ND ND ND ND
LEGEND:
Product stage
End-of-life stage
Benefits and loads beyond the system boundary
ND - not declared.
The impact indicator “POTENTIAL HUMAN EXPOSURE EFFICIENCY RELATIVE TO U235” focuses mainly on the possible impact of a low dose of ionising
radiation on human health resulting from the nuclear fuel cycle. It does not consider effects arising from possible nuclear accidents. occupational
exposure or the disposal of radioactive waste in underground facilities. Potential ionising radiation from soil. radon and some building materials is also
not measured by this indicator.
The results of the indicators “POTENTIAL COMPARATIVE TOXIC UNIT FOR ECOSYSTEMS (ETP-FW)”. “POTENTIAL COMPARATIVE TOXIC UNIT FOR
HUMANS. CANCER EFFECTS”. “POTENTIAL COMPARATIVE TOXIC UNIT FOR HUMANS. NOT CANCER EFFECTS” and “POTENTIAL SOIL QUALITY INDEX”
should be used with caution as the uncertainties associated with them are high or there is little experience with the indicator.
DAPHabitat System 11
2.4. Indicators describing resource use
Primary energy
EPR RR TRR EPNR RNR TRNR
Unit MJ. P.C.I. MJ. P.C.I. MJ. P.C.I. MJ. P.C.I. MJ. P.C.I. MJ. P.C.I.
Module A1-A3 1.35E+03 5.39E+01 1.40E+03 1.99E+04 4.56E+01 2.00E+04
Module C2 8.14E-01 0.00E+00 8.14E-01 3.12E+02 0.00E+00 3.12E+02
Module C3 1.69E+01 0.00E+00 1.69E+01 1.93E+02 0.00E+00 1.93E+02
Module C4 0.00E+00 0.00E+00 0.00E+00 0.00E+00 0.00E+00 0.00E+00
Module D -4.47E+02 0.00E+00 -4.47E+02 -7.51E+03 0.00E+00 -7.51E+03
LEGEND:
Product stage
End-of-life stage
Benefits and loads beyond the system boundary
EPR = use of renewable primary energy excluding renewable primary energy resources used as raw materials; RR = use of renewable primary energy
resources used as raw materials; TRR = total use of renewable primary energy resources (EPR + RR); EPNR = use of non-renewable primary energy
excluding non-renewable primary energy resources used as raw materials; RNR = use of non-renewable primary energy resources used as raw
materials; TRNR = total use of non-renewable primary energy resources (EPRN + RNR).
Values expressed per declared unit (1 t of cold-formed welded structural hollow sections).
Secondary materials and fuels, and use of water
MS CSR CSNR Net use of fresh water
Unit kg MJ. P.C.I. MJ. P.C.I. m3
Module A1-A3 4.37E+02 0.00E+00 0.00E+00 7.17E+00
Module C2 0.00E+00 0.00E+00 0.00E+00 1.31E-02
Module C3 0.00E+00 0.00E+00 0.00E+00 3.52E-02
Module C4 0.00E+00 0.00E+00 0.00E+00 0.00E+00
Module D 6.01E+02 0.00E+00 0.00E+00 -2.50E+00
LEGEND:
Product stage
End-of-life stage
Benefits and loads beyond the system boundary
MS = use of secondary material; CSR = use of renewable secondary fuels; CSNR = use of non-renewable secondary fuels.
Values expressed per declared unit (1 t of cold-formed welded structural hollow sections).
DAPHabitat System 12
2.5. Other environmental information describing different waste categories
Hazardous waste disposed Non-hazardous waste disposed Radioactive waste disposed
Unit kg kg kg
Module A1-A3 6.97E-01 0.00E+00 0.00E+00
Module C2 - - -
Module C3 - - -
Module C4 0.00E+00 0.00E+00 0.00E+00
Module D - - -
LEGENDA:
Product stage
End-of-life stage
Benefits and loads beyond the system boundary
Values expressed per declared unit (1 t of cold-formed welded structural hollow sections).
2.6. Environmental information describing output flows
Materials for energy
Components for re-use Materials for recycling Exported energy
recovery
Unidade kg kg kg MJ
Module A1-A3 0.00E+00 3.82E+01 0.00E+00 0.00E+00
Module C2 - - - -
Module C3 0.00E+00 1.00E+03 0.00E+00 0.00E+00
Module C4 0.00E+00 0.00E+00 0.00E+00 0.00E+00
Module D - - - -
LEGENDA:
Product stage
End-of-life stage
Benefits and loads beyond the system boundary
Values expressed per declared unit (1 t of cold-formed welded structural hollow sections).
DAPHabitat System 13
2.7. Information describing the biogenic carbon content at the factory gate
Biogenic carbon content* Units Modules A1-A3 (results)
Biogenic carbon content in product kg C 0
Biogenic carbon content in accompanying packaging kg C 0.720
* 1 kg biogenic carbon is equivalent to 44/12 kg of CO2.
Values expressed per declared unit (1 t of cold-formed welded structural hollow sections).
3. SCENARIOS AND ADDITIONAL TECHNICAL INFORMATION
3.1. C2 Transport – End-of-life of the product
Results expressed per
Parameter Units
declared unit
Vehicle type - Truck >32 t, EURO 5
Distance km 300
Average load of the truck t 16
3.2. C3 Waste processing for reuse. recovery and/or recycling – End-of-life of the product
Results expressed per
Parameter Units
declared unit
Material for re-use kg 0
Material for recycling kg 1,000
Material for energy recovery kg 0
3.3. C4 Disposal – End-of-life of the product
Results expressed per
Parameter Units
declared unit
Material for final deposition kg 0
3.4. Scenario and technical information for module D
Results expressed per declared unit
Parameter Units
Structural hollow sections at the end-
Scrap from the manufacturing process
of-life
Net output flow of steel scrap kg 579 22.0
Steel avoided production kg 515 19.4
Location of end-of-waste point - At the scrap sorting plant.
Steel manufactured from scrap is considered to have the same quality as steel
Point of functional equivalence -
manufactured from primary material.
The net output flow of steel scrap is calculated by the difference between the flow
Assumptions - of steel scrap that will be recycled and the input flow of steel scrap used in the steel
consumed in the manufacturing of the structural hollow sections.
DAPHabitat System 14
3.5. Additional information on release of dangerous substances to indoor air, soil, and
water during the use stage
Not applicable.
4. REFERENCES
✓ General Instructions of the DAPHabitat System. Version 2.1. Edition August 2023 (in www.daphabitat.pt);
✓ PCR – basic module for construction products and services. DAPHabitat System. Version 2.3. August 2023 (in
www.daphabitat.pt);
✓ ISO 14025:2009 Environmental declarations and labels – Type III environmental declarations – Principles and
procedures;
✓ EN 15804:2012 + A2:2019 Sustainability of construction works – Environmental product declarations – Core
rules for the product category of construction products;
✓ EN 15942:2021 Sustainability of construction works – Environmental product declarations – Communication
format business-to-business.
DAPHabitat System 15
