ENVIRONMENTAL PRODUCT DECLARATION
as per ISO 14025 and EN 15804+A2
Owner of the Declaration ARGE – The European Federation of Locks and Building Hardware Manufacturers
Publisher Institut Bauen und Umwelt e.V. (IBU)
Programme holder Institut Bauen und Umwelt e.V. (IBU)
Declaration number EPD-ARG-20230551-IBG1-EN
Issue date 02.04.2024
Valid to 01.04.2029
Shutter hardware
ARGE – The European Federation of Locks
and Building Hardware Manufacturers
This EPD is valid only for products supplied by an ARGE EPD licence holder.
www.ibu-epd.com | https://epd-online.com
1. General Information
ARGE – The European Federation of Locks Shutter hardware
and Building Hardware Manufacturers
Programme holder Owner of the declaration
IBU – Institut Bauen und Umwelt e.V. ARGE – The European Federation of Locks and Building Hardware
Hegelplatz 1 Manufacturers
10117 Berlin Offerstraße 12
Germany 42551 Velbert
Germany
Declaration number Declared product / declared unit
EPD-ARG-20230551-IBG1-EN 1 kg of shutter hardware
This declaration is based on the product category rules: Scope:
Building Hardware products, 01.08.2021 This ARGE EPD covers shutter hardware designed to be integrated into
(PCR checked and approved by the SVR) shutter assemblies of varying materials and applications. The reference
product used to calculate the impact this product group has on the
environment is an item of shutter hardware composed primarily of
Issue date aluminium and Zamak and has been selected for the LCA (Life Cycle
Assessment) because it is the product with the highest impact for 1 kg of
02.04.2024
product. A validity scope analysis has also been carried out to determine
the limiting factors for shutter hardware covered by this EPD. In a
preliminary study (simplified LCA), it has been confirmed that this EPD
Valid to
represents the worst-case condition and it can therefore be used to cover
01.04.2029 all shutter hardware manufactured in Europe by ARGE member
companies.
The owner of the declaration shall be liable for the underlying information
and evidence; the IBU shall not be liable with respect to manufacturer
information, life cycle assessment data and evidences.
The EPD was created according to the specifications of EN 15804+A2. In
the following, the standard will be simplified as EN 15804.
Verification
The standard EN 15804 serves as the core PCR
Independent verification of the declaration and data according to ISO
Dipl.-Ing. Hans Peters
14025:2011
(Chairman of Institut Bauen und Umwelt e.V.)
internally X externally
Florian Pronold Dr. Matthew Fishwick,
(Managing Director Institut Bauen und Umwelt e.V.) (Independent verifier)
1 Environmental Product Declaration - ARGE – The European Federation of Locks and Building Hardware Manufacturers - Shutter hardware
2. Product
2.1 Product description/Product definition Brass is an alloy of zinc and copper. Components made of
This EPD covers all types of shutter hardware used to ensure brass are made by extrusion, forging, die-casting or other types
the correct operation of shutters in buildings. It includes hinges of mechanical processing.
and fasteners.
For the application and use the respective national provisions Stainless steel is produced by combining iron with chromium
apply. as well as other elements depending on the desired
characteristics. Components made of steel are formed by
2.2 Application
stamping or other types of mechanical processing.
These products are designed to be integrated into shutter
assemblies consisting of various materials and used for various Steel is produced by combining iron with carbon as well as
applications. Their purpose is to ensure the correct operation of other elements depending on the desired characteristics.
the shutters. They may be used for either interior or exterior Components made of steel are formed by stamping or other
shutters. types of mechanical processing.
2.3 Technical Data
1) This product/article/at least one partial article contains
Ideally, products should comply with a suitable technical
substances listed in the ECHA candidate list (date: 14.06.2023)
specification. EN 14648:2007, Building hardware – Fittings for
exceeding 0.1 percentage by mass: Certain components may
shutters – Requirements and test methods is an example of
contain small amounts of lead (CAS no. 7439-92-1) as an
such a specification and some products will comply with it. The
alloying element.
relevant grading structure is shown in the following table:
Name Value Unit
2) This product/article/at least one partial article contains other
Category of use - Grade cancerogenic, mutagenic, reprotoxic (CMR) substances in
Endurance 2, 3 Grade categories 1A or 1B which are not on the ECHA candidate list,
Mass of the shutter - Grade exceeding 0.1 percentage by mass: no.
Fire resistance 0 Grade
3) Biocide products were added to this construction product or it
Safety of operators during use 1 Grade
has been treated with biocide products (this then concerns a
Corrosion resistance 4 Grade treated product as defined by the (EU) Ordinance on Biocide
Products No. 528/2012): no.
Performance data of the product with respect to its
characteristics in accordance with the relevant technical
2.6 Manufacture
provision (no CE-marking).
The production of a shutter hardware device usually follows a
2.4 Delivery status 3-step procedure:
The products are sold by unit. Deliveries of individual items are 1. Manufacture of the components: this step may include
possible but are an exception. Standard deliveries comprise a surface treatment in the factory or by external
larger quantity of shutter hardware devices, as they are contractors.
marketed as "B2B" products and not to end-users. 2. Pre-assembly of modules (in the factory).
3. Final assembly (in the factory).
2.5 Base materials/Ancillary materials
Composition of product analysed for this EPD: 2.7 Environment and health during manufacturing
Regular measurements of air quality and noise levels are
The values given in the table below are for the product performed by ARGE member companies. The results shall be
analysed for this EPD. Ranges of values for other products within compulsory safety levels. In areas where employees are
covered by the validity scope analysis are shown in brackets. exposed to chemical products, prescribed safety clothes and
Name Value Unit technical safety devices shall be provided. Regular health
checks are mandatory for employees on production sites.
Aluminium (0.00% – 99.28%) 59 %
Zamak (0.00% – 33.64%) 33.64 % 2.8 Product processing/Installation
Nylon 66 (0.00% – 14.17%) 5.61 % The installation of the product could vary depending on the type
Brass (0.00% – 1.75%) 1.75 % of shutter and the specific situation but products shall not
require energy consumption for installation.
Stainless steel (0.00% – 20.00%) 0 %
Steel (0.00% – 100.00%) 0 % 2.9 Packaging
Aluminium is a non-ferrous metal produced from bauxite by Normally, each individual product is packed in paper or
the Bayer process. Components made of aluminium are cardboard. These individual products are then packed in a
manufactured by extrusion or other types of mechanical cardboard box and stacked on wooden pallets for transport to
processing. the customer.
Zamak is an alloy with a base metal of zinc and alloying Waste from product packaging is collected separately for waste
elements of aluminium, magnesium, and copper. Components disposal (including recycling).
made of Zamak are die-cast.
2.10 Condition of use
Nylon 66 is a polymer, in particular polyamide. It is formed by Once installed, the products shall require no servicing during
the polycondensation of hexamethylenediamine and adipic acid their expected service lives. There shall be no consumption of
in equal parts. Components made of Nylon 66 are formed by water or energy linked to their use, and they shall not cause
injection moulding or other thermal forming processes. any emissions.
2 Environmental Product Declaration - ARGE – The European Federation of Locks and Building Hardware Manufacturers - Shutter hardware
hazardous substances in the event of flooding.
2.11 Environment and health during use
No environmental damage or health risks are to be expected Mechanical destruction
during normal conditions of use. Mechanical destruction of the declared product shall not
materially alter its composition or have any adverse effect on
2.12 Reference service life
the environment.
The reference service life is 30 years under normal working
conditions. This corresponds to passing a mechanical 2.14 Re-use phase
endurance test of 10.000 cycles as specified in EN 14648. The Removal of shutter hardware (for re-use or recycling) shall have
reference service life is dependent on the actual frequency of no adverse effect on the environment.
use and environmental conditions. It is required that installation,
as well as maintenance of the product, must be done in line 2.15 Disposal
with instructions provided by the manufacturer. Shutter hardware should be re-cycled wherever possible,
providing that there is no adverse effect on the environment.
2.13 Extraordinary effects The waste code in accordance with the European Waste Code
Fire is 17 04 07.
There are no specific fire resistance requirements.
2.16 Further information
Water Details of all types and variants can be found on the
The declared product is intended to be used in buildings under manufacturers' websites. The respective website addresses are
normal conditions (indoor or outdoor use). It shall not emit available at https://arge.org.
3. LCA: Calculation rules
• when a material is sent for recycling, generic transport
3.1 Declared Unit
and electric consumption of a shredder is taken into
The declared unit for all products covered by ARGE EPD is 1
account (corresponding to the process 'Grinding,
kg (of product). Since individual products will rarely weigh
metals'). Only then, is the material considered to have
exactly 1 kg it is necessary to establish the exact weight of the
attained the 'end-of-waste' state.
product and then use this as a correction factor to determine
• each type of waste is modelled as a transport to the
the true values for 1 kg of product in the tables (Section 5).
treatment site with a distance of 30 km. Parts sent for
Declared unit recycling include electricity consumption (grinding) and
Name Value Unit a flow ('Materials for recycling, unspecified').
Declared unit 1 kg
3.3 Estimates and assumptions
Mass of declared product 0.571 kg
The LCA data of the declared product had been calculated from
Raw density 1 kg/m3 the production data of one ARGE member company having
nine different products. This company had been chosen by
ARGE as being representative by virtue of its production
3.2 System boundary processes and market share. The chosen product follows the
Type of the EPD: "cradle to gate with options, with modules C1 "worst-case" principle as explained in Section 6 - LCA
– C4, and module D (A1-A3, C1-C3, D and additional interpretation.
modules)"
3.4 Cut-off criteria
The cut-off criteria considered are 1% of renewable and non-
The analysis of the product life cycle includes the production
renewable primary energy usage and 1% of the total mass of
and transport of the raw materials, the manufacture of the
that unit process. The total neglected input flows per module
product and the packaging materials which are declared in
shall be a maximum of 5% of energy usage and mass.
modules A1-A3.
Losses during production are considered as waste and are sent
For this study, all input and output flows have been considered
for recycling. No recycling processes are taken into account
at 100%, including raw materials as per the product
except for transport and an electricity consumption for grinding
composition provided by the manufacturer and packaging of
the metals. When recycled metals are used as raw material
raw materials as well as the final product. Energy and water
only their transformation process is taken into account and not
consumptions have also been considered at 100% according to
the extraction of the raw material.
the data provided.
A4 module represents the transport of the finished shutter
hardware to the installation site.
With the approach chosen, no significant environmental
There is no waste associated with the installation of the
impacts are known to have been cut off.
product. The A5 module therefore represents only the disposal
of the product packaging.
3.5 Background data
The End-of-Life (EoL) stages are also considered. The
For the life cycle modelling of the considered product, all
transportation to the EoL disposal site is taken into account in
relevant background datasets are taken from ecoinvent v3.8
module C2. Module C4 covers the disposal of the locks. Module
(system model: cut-off by classification).
C3 covers the recycling of the individual elements according to
European averages, with the remaining waste divided between 3.6 Data quality
incineration and landfill. Such a mixed scenario is declared due
The objective of this evaluation is to evaluate the environmental
to the complex material mix of the product and the dependency
impacts generated by the products throughout their entire life
of the EoL-route on the EoL-route of the product the shutter
cycles. To this end, ISO 14040, ISO 14044 and EN 15804 have
hardware has been integrated into.
been met regarding the quality of data on the following different
In practice, the end of life has been modelled as follows:
criteria:
3 Environmental Product Declaration - ARGE – The European Federation of Locks and Building Hardware Manufacturers - Shutter hardware
Time: The life cycle inventory data used come from: 3.8 Geographic Representativeness
Land or region, in which the declared product system is
• Data collected specifically for this study on the ARGE
manufactured, used or handled at the end of the product´s
member companies' manufacturing sites. Datasets are
lifespan: Europe
based on 1-year averaged data (time period: January
2013 to December 2013 considered representative for
2022). 3.9 Allocation
• In the absence of collected data, generic data from the
The products covered by this EPD are produced on one
ecoinvent v3.8 database have been used. This is
production site. All data were provided by the manufacturer of
updated regularly and is representative of current
the products per unit and then divided by the mass of the
processes (the entire database having been updated in
product to give a value per kg of product produced.
2021).
Geography: Data come from the production sites of the ARGE
The assumptions relating to the EoL of the product are
member companies. Generic data come from the ecoinvent
described in the section System Boundaries.
database, representative for European production processes.
3.10 Comparability
Technology: Material shaping technologies are based on Basically, a comparison or an evaluation of EPD data is only
European technology in the case of the use of generic data. possible if all the data sets to be compared were created
according to EN 15804 and the building context, respectively
A total of 9 typical products (based on sales figures) have been the product-specific characteristics of performance, are taken
evaluated, and the worst-case results are used in the tables. into account.
3.7 Period under review
ecoinvent v3.8 (system model: cut-off by classification) has
The data of the LCA is based on the annual production data of
been used as the background database.
an ARGE member from 2013, considered representative for the
year 2022.
4. LCA: Scenarios and additional technical information
It is assumed that a 16–32-ton truck is used to transport the
Characteristic product properties of biogenic carbon
product:
- Transport to shredding facility for metal recovery: 150 km
Information on the biogenic carbon content at factory gate - Transport to municipal waste incineration plant: 50 km
- Transport to landfill: 30 km
Note: 1 kg of biogenic carbon is equivalent to 44/12 kg of CO .
2
Name Value Unit Reuse, recovery and/or recycling potentials (D), relevant
kg scenario information
Biogenic carbon content in product 0
C
Biogenic carbon content in accompanying kg Module D contains the benefits and loads beyond the system
0.0570
packaging C boundary related to the recycling of metals, which result from
the treatment of recycled materials from the point of end-of-
waste status to the point of substitution (as costs) and the
The following information is the basis of the declared modules
substitution of primary resources (as benefits).
within the LCA in this EPD.
Transport to the building site (A4) According to EN 16710, clause 6.4.3.3: 'In module D
Name Value Unit substitution effects are calculated only for the resulting net
output flow.
Litres of fuel 25.8 l/100km
Transport distance 3500 km
For building hardware, the following rules apply for the
Capacity utilisation (including empty runs) 36 % quantification of net output flows:
- all production scrap and cuttings leave modules A1-B3 as
Installation into the building (A5)
sorted scrap without allocated burdens from primary production;
Name Value Unit the corresponding amounts are declared as material for
Material loss 0.144 kg recycling (MFR);
- net amounts of a metal leaving the product system are
quantified as the material for recycling leaving modules A1-C4
Reference service life minus the input of secondary scrap (secondary material, SM) to
Name Value Unit the product system
- in the case of brass and zinc alloys, which are composed of
Reference service life (condition of use: see
30 a two different constituting metals, no difference shall be made
§2.13)
between the input of secondary constituting metals (Cu and Zn;
Test cycles over RSL (EN 14648) 10'000 cycles
Cu and Sn) and its alloys (CuZn; CuSn).
Negative net output flows have been considered in the
End of life (C1-C4)
quantification of module D.
Name Value Unit
Collected separately waste type 1 kg It also includes the benefits and loads related to 'exported
Recycling 0.32 kg energy electricity' and 'exported energy heat' resulting from the
Energy recovery 0.313 kg energy recovery from plastic wastes in a municipal waste
incineration plant as modelled in Modules A3, A5 and C4.
Landfilling 0.367 kg
4 Environmental Product Declaration - ARGE – The European Federation of Locks and Building Hardware Manufacturers - Shutter hardware
5. LCA: Results
In Table 1 "Description of the system boundary", the declared modules are indicated with an "X"; all modules that are not declared
within the EPD but where additional data are available are indicated with "MND". Those data can also be used for building assessment
scenarios. The values are declared with three valid digits in exponential form.
The set of characterisation factors EF3.0 has been used for the life cycle assessment.
DESCRIPTION OF THE SYSTEM BOUNDARY (X = INCLUDED IN LCA; MND = MODULE OR INDICATOR NOT DECLARED; MNR
= MODULE NOT RELEVANT)
Benefits and
Construction loads beyond
Product stage Use stage End of life stage
process stage the system
boundaries
la ire wta am R y lp p u s tro p s n a rT g n iru tc a fu n a M tro p s nm ae o rh r
T
f te tis e h t o t e ta g y lb m e s s A e s U e c n a n e tn ia M ria p e R tn e m e c a lp e R tn e m h s ib ru fe R la n o ity ag rr ee pn Oe e s u la n o ita r re et pa Ow e s u n o itc u rts n eo Dc -n o itilo m e d tro p s n a rT g n is s ee tsc ao Wrp la s o p s iD e s u e R- y re v o c e R- g n ilc y c e R- la itn e to p
A1 A2 A3 A4 A5 B1 B2 B3 B4 B5 B6 B7 C1 C2 C3 C4 D
X X X X X MND MND MNR MNR MNR MND MND X X X X X
RESULTS OF THE LCA - ENVIRONMENTAL IMPACT according to EN 15804+A2: 1 kg of shutter hardware device
Parameter Unit A1-A3 A4 A5 C1 C2 C3 C4 D
GWP-total kg CO2 eq 1.39E+01 6.52E-01 2.32E-01 0 1.52E-02 3.19E-03 4.99E-02 -3.18E+00
GWP-fossil kg CO2 eq 1.41E+01 6.52E-01 2.33E-02 0 1.51E-02 3.18E-03 4.99E-02 -3.17E+00
GWP-biogenic kg CO2 eq -2.09E-01 0 2.09E-01 0 0 0 0 0
GWP-luluc kg CO2 eq 3.73E-02 2.61E-04 1.24E-06 0 6.06E-06 7.93E-06 4.06E-06 -1.21E-02
ODP kg CFC11 eq 5.76E-07 1.51E-07 6.91E-10 0 3.51E-09 1.61E-10 1.74E-09 -1.07E-07
AP mol H+ eq 1.09E-01 1.85E-03 1.72E-05 0 4.3E-05 1.64E-05 5.16E-05 -1.84E-02
EP-freshwater kg P eq 6.02E-04 4.65E-06 2.96E-08 0 1.08E-07 3.57E-07 1E-07 -9.35E-05
EP-marine kg N eq 1.51E-02 3.68E-04 6.11E-06 0 8.55E-06 2.1E-06 2.15E-05 -2.9E-03
EP-terrestrial mol N eq 1.66E-01 4.1E-03 6.6E-05 0 9.53E-05 2.43E-05 2.1E-04 -3.21E-02
kg NMVOC
POCP 4.81E-02 1.58E-03 1.85E-05 0 3.66E-05 6.64E-06 6.06E-05 -9.62E-03
eq
ADPE kg Sb eq 1.11E-03 2.31E-06 1.14E-08 0 5.37E-08 7.7E-09 2.82E-08 3.87E-04
ADPF MJ 1.45E+02 9.89E+00 4.76E-02 0 2.3E-01 6.74E-02 1.23E-01 -2.74E+01
m3 world eq
WDP 2.84E+00 3.01E-02 3E-04 0 6.99E-04 7.53E-04 -7.27E-04 -2.96E-01
deprived
GWP = Global warming potential; ODP = Depletion potential of the stratospheric ozone layer; AP = Acidification potential of land and water; EP =
Eutrophication potential; POCP = Formation potential of tropospheric ozone photochemical oxidants; ADPE = Abiotic depletion potential for non-fossil
resources; ADPF = Abiotic depletion potential for fossil resources; WDP = Water (user) deprivation potential)
RESULTS OF THE LCA - INDICATORS TO DESCRIBE RESOURCE USE according to EN 15804+A2: 1 kg of shutter hardware
device
Parameter Unit A1-A3 A4 A5 C1 C2 C3 C4 D
PERE MJ 1.65E+01 1.39E-01 -7.08E-01 0 3.23E-03 1.28E-02 9.73E-03 -3.67E+00
PERM MJ 1.78E+00 0 -2.15E-01 0 0 0 0 0
PERT MJ 1.83E+01 1.39E-01 -9.23E-01 0 3.23E-03 1.28E-02 9.73E-03 -3.67E+00
PENRE MJ 1.44E+02 9.89E+00 3.38E-01 0 2.3E-01 6.8E-02 1.23E-01 -2.74E+01
PENRM MJ 1.46E+00 0 -2.9E-01 0 0 0 0 0
PENRT MJ 1.46E+02 9.89E+00 4.76E-02 0 2.3E-01 6.8E-02 1.23E-01 -2.74E+01
SM kg 2.63E-01 0 0 0 0 0 0 0
RSF MJ 0 0 0 0 0 0 0 0
NRSF MJ 0 0 0 0 0 0 0 0
FW m3 1.06E-01 1.05E-03 5.19E-05 0 2.44E-05 4.34E-05 2.39E-04 -1.68E-02
PERE = Use of renewable primary energy excluding renewable primary energy resources used as raw materials; PERM = Use of renewable primary
energy resources used as raw materials; PERT = Total use of renewable primary energy resources; PENRE = Use of non-renewable primary energy
excluding non-renewable primary energy resources used as raw materials; PENRM = Use of non-renewable primary energy resources used as raw
materials; PENRT = Total use of non-renewable primary energy resources; SM = Use of secondary material; RSF = Use of renewable secondary fuels;
NRSF = Use of non-renewable secondary fuels; FW = Use of net fresh water
RESULTS OF THE LCA – WASTE CATEGORIES AND OUTPUT FLOWS according to EN 15804+A2:
1 kg of shutter hardware device
Parameter Unit A1-A3 A4 A5 C1 C2 C3 C4 D
HWD kg 1.57E-03 2.58E-05 2.15E-07 0 5.99E-07 2.39E-08 2.23E-07 5.5E-04
NHWD kg 3.49E+00 5.2E-01 3.19E-03 0 1.21E-02 2.53E-04 3.99E-01 -9.22E-01
RWD kg 6.17E-04 1.43E-04 6.17E-07 0 3.32E-06 9.06E-07 1.56E-06 -8E-05
CRU kg 0 0 0 0 0 0 0 0
MFR kg 1.89E-01 0 9.3E-02 0 0 4.76E-01 0 0
5 Environmental Product Declaration - ARGE – The European Federation of Locks and Building Hardware Manufacturers - Shutter hardware
MER kg 0 0 0 0 0 0 0 0
EEE MJ 5.02E-03 0 3.71E-02 0 0 0 2.51E-02 0
EET MJ 3.33E-02 0 2.45E-01 0 0 0 1.67E-01 0
HWD = Hazardous waste disposed; NHWD = Non-hazardous waste disposed; RWD = Radioactive waste disposed; CRU = Components for re-use;
MFR = Materials for recycling; MER = Materials for energy recovery; EEE = Exported electrical energy; EET = Exported thermal energy
RESULTS OF THE LCA – additional impact categories according to EN 15804+A2-optional:
1 kg of shutter hardware device
Parameter Unit A1-A3 A4 A5 C1 C2 C3 C4 D
Disease
PM 1.1E-06 5.24E-08 3E-10 0 1.22E-09 4.38E-11 1.17E-09 -2.81E-07
incidence
IR kBq U235 eq 3.06E-01 4.29E-02 1.88E-04 0 9.97E-04 6.14E-04 5.91E-04 -2.46E-02
ETP-fw CTUe 5.84E+02 7.76E+00 4.49E-02 0 1.8E-01 3.39E-02 8.48E+01 -1.15E+01
HTP-c CTUh 2.6E-08 2.5E-10 3.37E-12 0 5.8E-12 9.06E-13 2.11E-11 9.1E-11
HTP-nc CTUh 9.12E-07 7.84E-09 1.37E-10 0 1.82E-10 2.94E-11 2.46E-10 1.41E-07
SQP SQP 6.01E+01 6.89E+00 3.03E-02 0 1.6E-01 1.04E-02 2.1E-01 -5.16E-01
PM = Potential incidence of disease due to PM emissions; IR = Potential Human exposure efficiency relative to U235; ETP-fw = Potential comparative
Toxic Unit for ecosystems; HTP-c = Potential comparative Toxic Unit for humans (cancerogenic); HTP-nc = Potential comparative Toxic Unit for humans
(not cancerogenic); SQP = Potential soil quality index
Disclaimer 1 – for the indicator 'Potential Human exposure efficiency relative to U235'. This impact category deals mainly with the
eventual impact of low-dose ionizing radiation on human health of the nuclear fuel cycle. It does not consider effects due to possible
nuclear accidents, occupational exposure or radioactive waste disposal in underground facilities. Potential ionizing radiation from the
soil, radon and from some construction materials is also not measured by this indicator.
Disclaimer 2 – for the indicators 'abiotic depletion potential for non-fossil resources', 'abiotic depletion potential for fossil resources',
'water (user) deprivation potential, deprivation-weighted water consumption', 'potential comparative toxic unit for ecosystems', 'potential
comparative toxic unit for humans – cancerogenic', 'Potential comparative toxic unit for humans - not cancerogenic', 'potential soil
quality index'. The results of this environmental impact indicator shall be used with care as the uncertainties on these results are high
as there is limited experience with the indicator.
6. LCA: Interpretation
Figure 1 illustrates the relative contributions of the different
modules along the life cycle of the declared products.
Figure 1: Environmental impacts of shutter hardware along Benefits and burdens beyond the system boundary (module D)
its life cycle are in the order of 5 % to 20 % of the impacts over the product
life cycle (modules A1-A3) and relate basically to the recycling
The largest part of environmental impacts is caused during of metals; module. Only for ADPelements, the negative net
production (modules A1-A3); comparably small impacts are amount of zinc leaving the product system leads to additional
caused during the transport of the product to the construction burdens in module D from the compensation of material losses
site (via the manufacturer of the product, which the shutter with primary production of zinc.
hardware has been integrated into). A total of 9 typical products (based on sales figures) have been
evaluated and the worst-case results are used in section 5 of
All the other modules related to the product life cycle are not this EPD. In chapter 2.5, the tabulated range of relative weight
significant. per material ensures that the variability of results stays within
6 Environmental Product Declaration - ARGE – The European Federation of Locks and Building Hardware Manufacturers - Shutter hardware
+/- 40% of the declared values (assessed for the indicators GWP, PENRT, and non-hazardous waste).
7. Requisite evidence
No testing results are required by the PCR part B.
8. References
Product category rules of IBU 14044:2006.
IBU (2021) EN 14648
IBU (2021): General Instructions for the EPD Programme of the EN 14648:2007, Building hardware - Fittings for shutters -
Institut Bauen und Umwelt e.V. (General Instructions for the Requirements and test methods.
IBU EPD Programme). Version 2.0, Institut Bauen und Umwelt,
Berlin. ISO 15686
ISO 15686:1, -2, -7 and -8. Service life planning (various parts).
IBU (2021)
IBU (2021): PCR Part A: Calculation rules for the life cycle ECHA candidate list
assessment and requirements on the project report according Candidate List of substances of very high concern for
to EN 15804+A2. Version 1.3., Institut Bauen und Umwelt, Authorisation, published in accordance with Article 59(10) of the
Berlin. REACH Regulation. European Chemicals Agency, Brussels.
IBU (2023) Ordinance on Biocide Products No. 528/2012
IBU (2023): PCR Part B: Requirements on the EPD for building REGULATION (EU) No 528/2012 OF THE EUROPEAN
hardware products, Institut Bauen und Umwelt, Berlin. PARLIAMENT AND OF THE COUNCIL of 22 May 2012
concerning the making available on the market and use of
Standards and legal documents biocidal products.
EN 15804 European List of Waste
EN 15804:2012+A2:2019+AC:2021, Sustainability of Commission Decision of 3 May 2000 replacing Decision
construction works - Environmental product declarations - Core 94/3/EC establishing a list of wastes pursuant to Article 1(a) of
rules for the product category of construction products. Council Directive 75/442/EEC on waste and Council Decision
94/904/EC establishing a list of hazardous waste pursuant to
EN 17610 Article 1(4) of Council Directive 91/689/EEC on hazardous
EN 17610:2022, Building hardware - Environmental product waste (notified under document number C(2000) 1147).
declarations - Product category rules complementary to EN
15804 for building hardware. Additional references
ISO 14025 BBSR 2017
ISO 14025:2006-07, Environmental labels and declarations - BBSR (2017): Nutzungsdauer von Bauteilen in
Type III Environmental declarations - Principles and Lebenszyklusanalysen nach Bewertungssystem Nachhaltiges
procedures. Bauen (BNB). Version vom 24.10.2017, Bundesinstitut für Bau-,
Stadt- und Raumforschung, Berlin.
ISO 14044
EN ISO 14044:2006-07, Environmental management - Life ecoinvent v3.8
cycle assessment - Requirements and guidance (ISO http://www.ecoinvent.org
14044:2006); German and English versions EN ISO
7 Environmental Product Declaration - ARGE – The European Federation of Locks and Building Hardware Manufacturers - Shutter hardware
Publisher
Institut Bauen und Umwelt e.V. +49 (0)30 3087748- 0
Hegelplatz 1 info@ibu-epd.com
10117 Berlin www.ibu-epd.com
Germany
Programme holder
Institut Bauen und Umwelt e.V. +49 (0)30 3087748- 0
Hegelplatz 1 info@ibu-epd.com
10117 Berlin www.ibu-epd.com
Germany
Author of the Life Cycle Assessment
Dr. Frank Werner - Umwelt & Entwicklung + 41 (0)44 241 39 06
Kammelenbergstrasse 30 frank@frankwerner.ch
9011 St. Gallen http://www.frankwerner.ch/
Switzerland
Owner of the Declaration
ARGE – The European Federation of Locks and +49 (0)2051 9506 15
Building Hardware Manufacturers mail@arge.org
Offerstraße 12 www.arge.org
42551 Velbert
Germany
8 Environmental Product Declaration - ARGE – The European Federation of Locks and Building Hardware Manufacturers - Shutter hardware
