ENVIRONMENTAL PRODUCT DECLARATION
as per ISO 14025 and EN 15804+A2
Owner of the Declaration Hansgrohe Group
Publisher Institut Bauen und Umwelt e.V. (IBU)
Programme holder Institut Bauen und Umwelt e.V. (IBU)
Declaration number EPD-HAN-20240194-ICC1-EN
Issue date 26.09.2024
Valid to 25.09.2029
Washbasins
Hansgrohe Group
www.ibu-epd.com | https://epd-online.com
1. General Information
Hansgrohe Group Washbasins
Programme holder Owner of the declaration
IBU – Institut Bauen und Umwelt e.V. Hansgrohe Group
Hegelplatz 1 Auestr. 5-9
10117 Berlin 77761 Schiltach
Germany Germany
Declaration number Declared product / declared unit
EPD-HAN-20240194-ICC1-EN One piece of an average ceramic washbasin incl. packaging
This declaration is based on the product category rules: Scope:
Sanitary ceramics, 01.08.2021 This average EPD is valid for the product group of ceramic washbasins of
(PCR checked and approved by the SVR) the hansgrohe brand sold on the European market. The products are
produced in Italy and Egypt.
The owner of the declaration shall be liable for the underlying information
Issue date and evidence; the IBU shall not be liable with respect to manufacturer
information, life cycle assessment data and evidences.
26.09.2024
The EPD was created according to the specifications of EN 15804+A2. In
the following, the standard will be simplified as EN 15804.
Valid to
25.09.2029 Verification
The standard EN 15804 serves as the core PCR
Independent verification of the declaration and data according to ISO
14025:2011
internally X externally
Dipl.-Ing. Hans Peters
(Chairman of Institut Bauen und Umwelt e.V.)
Florian Pronold Dr Naeem Adibi,
(Managing Director Institut Bauen und Umwelt e.V.) (Independent verifier)
1 Environmental Product Declaration - Hansgrohe Group - Washbasins
2. Product
Name Value Unit
2.1 Product description/Product definition
Ceramic 78 - 94 %
The product group of washbasins refers to ceramic articles in
Steel 0 - 7 %
various sizes and designs.
Plastic < 1 %
The basic material of ceramics consists of natural raw materials Other 0 - 6 %
such as clay, kaolin, quartz and feldspar that are mixed Cardboard and paper (packaging) 5 - 15 %
according to a specific recipe. A glaze protects the products
Polyethylene (packaging) 0 - 2 %
from external influences.
The parts which are made of brass contain between 1.6 and
Depending on the model, additional components (e. g. made of 2.5% lead.
porcelain, plastic or metals) may be included in the scope of This product contains substances listed in the candidate list
delivery. (date: 12.12.2023) exceeding 0.1 percentage by mass: Lead
For the placing on the market of the product in the European (CAS number 7439-92-1) as a component of the brass alloy
Union/European Free Trade Association (EU/EFTA) (with the has been on the candidate list of the Reach Regulation
exception of Switzerland) Regulation (EU) No. 305/2011 (CPR) (Regulation (EC) No. 1907/2006) since 27.06.2018.
applies. The product needs a declaration of performance taking
into consideration This product/article/at least one partial article contains other
CMR substances in categories 1A or 1B which are not on the
• EN 14688:2006, sanitary appliances -wash basins -
candidate list, exceeding 0.1 percentage by mass: no.
functional requirements and test methods
and the CE-marking.
Biocide products were added to this construction product or it
has been treated with biocide products (this then concerns a
For the application and use the respective national provisions
treated product as defined by the (EU) Ordinance on Biocide
apply.
Products No. 528/2012): yes.
In order to get the desired viscosity, fungicides are added to the
2.2 Application glaze. These burn completely during the firing process and are
not part of the final product.
As typical sanitary installations washbasins are part of the
bathroom and support the water-based physical hygiene. They
2.6 Manufacture
are combined with a fitting to provide the hygiene function.
2.3 Technical Data
Constructional data
Name Value Unit
300-
Width mm
1200
Length 250-480 mm
Height 130-190 mm
Maximum heat resistance temperature (if
1100 °C
relevant)
Vol.-
Maximum water absorption (if relevant) 6
%
Resistance to chemicals and staining passed -
Resistance to temperature change passed -
Performance data of the product in accordance with the
declaration of performance with respect to its essential
characteristics according to
• EN 14688:2006, sanitary appliances -wash basins -
functional requirements and test methods.
No. 1: The "slip" is prepared by mixing raw materials and water.
2.4 Delivery status No. 2: The moulds are made by gypsum.
The washbasins are delivered singularly packaged. The No. 3: The "slip" is filled into the moulds.
packaging is customized to the size of the product and No. 4: The pieces are drying.
supplies. The products with the smallest and the largest volume No. 5: Glaze is prepared.
have dimensions between 381x291x126 mm and No. 6: Glaze is applied.
1,226x536x161 mm. No. 7: The pieces are fired in the kiln.
No. 8: The pieces are inspected for any defects.
2.5 Base materials/Ancillary materials No. 8a: Some parts are reworked, e. g. by grinding certain
The material composition (incl. packaging and additional parts) areas.
of an washbasins are as follows: No. 8b: Some parts are refired.
No. 9: The products are packed.
2 Environmental Product Declaration - Hansgrohe Group - Washbasins
2.7 Environment and health during manufacturing 2.11 Environment and health during use
Hansgrohe SE tries to keep the impact on people and the Our products do not emission any contaminants or substances
environment as low as possible when manufacturing its that are harmful to the environment or health during the use
products. phase.
For example, state-of-the-art systems (e. g. kilns) are used in
the production process of sanitary ceramics and application of 2.12 Reference service life
the glaze is partially carried out by robots. The quality and durability of our washbasins is designed for a
In addition, all production sites are certified according to the product life of about 20 years. Which on average is
ISO 9001 (quality), KIWA and NF. approximately the duration of use by the consumers.
2.8 Product processing/Installation All products in the scope of this study have a 20-year warranty.
The installation of a washbasin can vary depending on the
installation type (Wall-hung basin / Undercounter basin / Above
counter basin / Wash bowl). Depending on the variant, fixing is 2.13 Extraordinary effects
carried out by means of mounting parts and silicone. At the Fire
end, sealing is done with silicone. Sanitary ceramics are classified as building material class A1
(non-combustible without combustible building materials) in
Wall-hung basin / Countertop basin: accordance with EN 13501-1.
• Make holes in the wall for the fixation of the washbasin Fire protection
(tool: drilling machine). Name Value
• Insert dowels and stick screws (tools: hexagonal offset
Building material class A1
screwdriver, wrench).
Burning droplets -
• Add the sound insulation mat.
Smoke gas development -
• Nuts and washers get attached (tool: wrench).
• The valve is inserted (tool: wrench).
• Sealing is done with silicone (tools: silicone syringe). Water
Undercounter basin: If a room in which the products offered by Hansgrohe are
• Silicone is applied to the washbasin (tools: silicone installed is flooded with water, the products are not affected in
syringe). their function.
• The basin is fixed to the furniture with mounting parts. There will be no environmental impact.
Above counter basin:
Mechanical destruction
• Silicone is applied to the furniture and washbasin (tools:
Minor mechanical damages have no effect on product function.
silicone syringe).
If the glazed surface of the ceramic is severely destroyed by a
• The washbasin is placed in the furniture.
mechanical stress and the glaze flakes off, there is a very small
• Sealing is done with silicone (tools: silicone syringe).
possibility of water uptake as usual with ceramic products. In
Wash bowl:
this event the products may need to be replaced.
• Silicone is applied to the furniture and washbasin (tools:
silicone syringe). 2.14 Re-use phase
• The basin is fixed to the furniture with mounting parts. The washbasins are not taken back by the manufacturer for the
• Sealing is done with silicone (tools: silicone syringe). purpose of reuse. Users can disassemble the products
repeatedly within the reference utilization period and reuse
2.9 Packaging them elsewhere.
For product protection the washbasins are individually packed
2.15 Disposal
in a printed cardboard box. The inlay of the packaging consists
The waste code of the product is AVV 17 01 03.
of folded cardboard or plastic bags, depending on the product.
Disassembly of the products consists of the same steps as
The packaging can be fully recycled. All packaged products fit
assembly, in reverse order. Due to the disassembly process,
on a reusable euro pallet.
the individual parts may be collected separately.
2.10 Condition of use The ceramic material will mostly be disposed via inert landfills.
To protect the washbasins and make them durable, the ceramic All metal components can be recycled (as scrap). All plastic
material is glazed. If used as intended, there are no unhealthy components have a high calorific value and can be sent for
contaminants caused by the sanitary ceramics. To ensure the thermal recycling.
longevity of the product, it should be cleaned regularly. In countries where no thermal recycling or substance recycling
is established, disposal takes place via the waste incineration
plant.
2.16 Further information
Additional information about our products can be found at
https://www.hansgrohe.com.
3. LCA: Calculation rules
3.1 Declared Unit Weighted averaging based on forecast sales volumes is chosen
The results of this EPD are valid for the following declared unit: as the basis for creating the environmental profile. 128 different
one (1) washbasin including packaging, used in accordance washbasins were considered.
with the manufacturer's recommendations for a 20-year life,
following the manufacturer's operating instructions.
3 Environmental Product Declaration - Hansgrohe Group - Washbasins
Declared unit
3.5 Background data
Name Value Unit The LCA software LCA for Experts 10.7 was used to model the
Declared unit 1 piece life cycle. The entire manufacturing process, as well as energy
Declared unit (ceramic mass) 0.0143 t consumption, were modelled on the basis of manufacturer-
specific data.
Mass (product) 14.558 kg
Mass (packaging) 1.128 kg
However, generic background datasets were used for the
upstream and downstream processes. The majority of the
3.2 System boundary
background datasets used were taken from the content version
This average EPD follows the EPD type "cradle to grave". The 2023.2 of the Sphera Managed LCA Content database.
following life cycle modules are declared: Ecoinvent Version 3.9.1 datasets were only used when suitable
datasets were not available.
Modules A1-A3
The product stage begins with considering the production of the 3.6 Data quality
necessary raw materials and energies, including all The data for the examined products was captured on the basis
corresponding upstream chains and the actual procurement of evaluations of internal production and environmental data,
transports. Furthermore, the entire manufacturing phase was the collection of LCA relevant data within the supply chain, as
mapped, including the treatment of production waste until the well as the evaluation of relevant data for the energy supply.
end-of-waste status (EoW) was reached. Location-specific The collected data were checked for plausibility and
electricity mixes were considered. consistency. Good representativity can be assumed.
Module A4 3.7 Period under review
Distribution transports (A4) to the customers were considered. Life cycle assessment data were collected for a 12-month
period in the years 2022 and 2023.
Module A5
3.8 Geographic Representativeness
This module covers the installation process with the
corresponding packaging waste generated that needs to be Land or region, in which the declared product system is
disposed of. manufactured, used or handled at the end of the product´s
lifespan: Global
Module B2
Maintenance expenses are declared in this module and consist
3.9 Allocation
of weekly cleaning expenses for these products.
For the production of the ceramic, supplier-data was gathered
for a 12-month period and then allocated to the products under
Module B1, B3-B7
consideration by weight. This applies to the material inputs and
These modules were considered, but evaluated as not relevant
outputs as well as energy demands.
and therefore considered as zero.
The composition of the products under consideration was
Modules C1-C4
modelled based on BOMs. Therefore, no further allocation was
The modules include the environmental impacts for dismantling
necessary.
and the treatment of the waste fractions until the end-of-waste
status (EoW) is reached, including the associated transports at
Allocation of co-production processes is not relevant.
the end of the product life cycle.
Recycled materials enter the product system without any loads
in the modules A1-A3 and therefore do not generate any
Module D
benefits in module D.
Identification of the benefits and costs of the product outside
Loads and benefits beyond the system boundary resulting from
the system boundary. For plastics, these consist of energy
production waste in module A1-A3 are cut-off.
credits from thermal utilization in the form of the average
European electricity mix or thermal energy from natural gas. 3.10 Comparability
Recycling of steel results in material credits.
Basically, a comparison or an evaluation of EPD data is only
possible if all the data sets to be compared were created
3.3 Estimates and assumptions
according to EN 15804 and the building context, respectively
For the incineration with energy recovery (thermal and electric)
the product-specific characteristics of performance, are taken
of waste, an r1 value of >0.6 is assumed. The net efficiency for
into account. The background database used is LCA for
the average waste incinerated is 44 %.
Experts content version 2023.2.
All products are assumed to be first shipped to the warehouse
and then shipped to the customers. This is a conservative
assumption since some products are shipped directly from the
manufacturing site to the customer. However, no reliable data is
available.
3.4 Cut-off criteria
The effect associated with the neglected mass shares is less
than 5 % of the effect categories per module. The minimum
limit of 1 % total mass and the use of renewable and non-
renewable primary energy is not exceeded.
4 Environmental Product Declaration - Hansgrohe Group - Washbasins
4. LCA: Scenarios and additional technical information
Installation into the building (A5)
Characteristic product properties of biogenic carbon
Name ValueUnit
Silicone 0.085 kg
Information on describing the biogenic carbon content at
factory gate Steel (mounting parts) 0.101 kg
Note: 1 kg of biogenic carbon is equivalent to 44/12 kg of CO . Thermoplast (mounting parts) 0.001
2
Output substances following waste treatment on
Name ValueUnit 1.128 kg
site (packaging materials)
kg
Biogenic carbon content in product -
C
Biogenic carbon content in accompanying kg Reference service life
0.462
packaging C Name Value Unit
Life Span according to the manufacturer 20 a
End of life (C1-C4)
Name Value Unit
Transport to the building site (A4)
Collected as mixed construction waste 14.558 kg
Name Value Unit
Recycling 0.135 kg
Transport distance (truck) 655 km
Landfilling 14.453 kg
Capacity utilisation (including empty runs) (truck) 55 %
Transport distance (ship) 2517 km Reuse, recovery and/or recycling potentials (D), relevant
scenario information
Name Value Unit
5 Environmental Product Declaration - Hansgrohe Group - Washbasins
5. LCA: Results
The LCA results of the module B2 are declared for the service life of 20 years.
DESCRIPTION OF THE SYSTEM BOUNDARY (X = INCLUDED IN LCA; MND = MODULE OR INDICATOR NOT DECLARED; MNR
= MODULE NOT RELEVANT)
Benefits and
Construction loads beyond
Product stage Use stage End of life stage
process stage the system
boundaries
la ire ta m w a Ry lp p u s tro p s n a rT g n iru tc a fu n a M e h t m o rf tro p s n a rTe tis e h t o t e ta g y lb m e s s A e s U e c n a n e tn ia M ria p e R tn e m e c a lp e R tn e m h s ib ru fe R y g re n e la n o ita re p Oe s u re ta w la n o ita re p Oe s u n o itc u rts n o c -e Dn o itilo m e d tro p s n a rT g n is s e c o rp e ts a W la s o p s iD -e s u e R-y re v o c e R-g n ilc y c e Rla itn e to p
A1 A2 A3 A4 A5 B1 B2 B3 B4 B5 B6 B7 C1 C2 C3 C4 D
X X X X X X X X X X X X X X X X X
RESULTS OF THE LCA - ENVIRONMENTAL IMPACT according to EN 15804+A2: 1 piece washbasin
Parameter Unit A1-A3 A4 A5 B1 B2 B3 B4 B5 B6 B7 C1 C2 C3 C4 D
GWP-total kg CO 2 eq 2.93E+011.43E+002.67E+00 0 2.51E+01 0 0 0 0 0 0 1.44E-01 2.16E-01 2.2E-01 -5.5E-02
GWP-fossil kg CO 2 eq 3.1E+01 1.42E+00 9.72E-01 0 1.9E+01 0 0 0 0 0 0 1.43E-01 2.15E-01 2.2E-01 -5.5E-02
GWP-
biogenic kg CO 2 eq -1.7E+00 0 1.7E+00 0 0 0 0 0 0 0 0 0 0 0 0
GWP-luluc kg CO 2 eq 3.18E-02 9.55E-03 9.34E-04 0 6.04E+00 0 0 0 0 0 0 1.32E-03 7.01E-04 6.73E-04 -3.59E-06
kg CFC11
ODP 2.33E-07 1.61E-13 4.31E-12 0 1.09E-06 0 0 0 0 0 0 1.86E-14 2.61E-12 5.59E-13 -4.33E-13
eq
AP mol H+ eq 1.03E-01 1.51E-02 2.81E-03 0 6.84E-02 0 0 0 0 0 0 6.11E-04 7.05E-04 1.55E-03 -6.89E-05
EP-
kg P eq 6.05E-04 3.86E-06 1.81E-06 0 5.9E-04 0 0 0 0 0 0 5.21E-07 7.96E-07 1.74E-06 -8.93E-08
freshwater
EP-marine kg N eq 3.16E-02 6.92E-03 6.69E-04 0 1.56E-02 0 0 0 0 0 0 2.87E-04 2.67E-04 3.99E-04 -2.01E-05
EP-terrestrial mol N eq 3.39E-01 7.62E-02 7.23E-03 0 1.85E-01 0 0 0 0 0 0 3.21E-03 2.92E-03 4.39E-03 -2.16E-04
kg
POCP NMVOC 8.25E-02 1.59E-02 2.2E-03 0 6.2E-02 0 0 0 0 0 0 5.55E-04 5.99E-04 1.2E-03 -5.61E-05
eq
ADPE kg Sb eq 3.72E-05 7.19E-08 1.79E-05 0 3.25E-05 0 0 0 0 0 0 9.45E-09 2.67E-08 1.01E-08 -3.95E-09
-1.02E
ADPF MJ 4.87E+021.88E+011.42E+01 0 4.64E+02 0 0 0 0 0 0 1.94E+003.97E+002.98E+00
+00
m3 world
WDP eq 2.23E+00 1.31E-02 2.13E-01 0 6.83E+00 0 0 0 0 0 0 1.72E-03 3.23E-02 2.34E-02 -5.24E-03
deprived
GWP = Global warming potential; ODP = Depletion potential of the stratospheric ozone layer; AP = Acidification potential of land and water; EP =
Eutrophication potential; POCP = Formation potential of tropospheric ozone photochemical oxidants; ADPE = Abiotic depletion potential for non-fossil
resources; ADPF = Abiotic depletion potential for fossil resources; WDP = Water (user) deprivation potential)
RESULTS OF THE LCA - INDICATORS TO DESCRIBE RESOURCE USE according to EN 15804+A2: 1 piece washbasin
Parameter Unit A1-A3 A4 A5 B1 B2 B3 B4 B5 B6 B7 C1 C2 C3 C4 D
PERE MJ 4.64E+011.04E+002.43E+01 0 9.9E+01 0 0 0 0 0 0 1.41E-01 1.85E+00 4.77E-01 -2.95E-01
-1.85E
PERM MJ 1.85E+01 0 0 0 0 0 0 0 0 0 0 0 0 0
+01
PERT MJ 6.5E+01 1.04E+005.75E+00 0 9.9E+01 0 0 0 0 0 0 1.41E-01 1.85E+00 4.77E-01 -2.95E-01
-1.02E
PENRE MJ 4.85E+021.89E+011.25E+01 0 4.64E+02 0 0 0 0 0 0 1.95E+003.98E+002.98E+00
+00
PENRM MJ 2.55E+00 0 1.78E+00 0 0 0 0 0 0 0 0 0 0 0 0
-1.02E
PENRT MJ 4.88E+021.89E+011.42E+01 0 4.64E+02 0 0 0 0 0 0 1.95E+003.98E+002.98E+00
+00
SM kg 9.43E-01 0 0 0 0 0 0 0 0 0 0 0 0 0 1.23E-01
RSF MJ 0 0 0 0 0 0 0 0 0 0 0 0 0 0 0
NRSF MJ 0 0 0 0 0 0 0 0 0 0 0 0 0 0 0
FW m3 6.67E-02 1.15E-03 7.69E-03 0 1.62E-01 0 0 0 0 0 0 1.55E-04 1.51E-03 7.22E-04 -2.39E-04
PERE = Use of renewable primary energy excluding renewable primary energy resources used as raw materials; PERM = Use of renewable primary
energy resources used as raw materials; PERT = Total use of renewable primary energy resources; PENRE = Use of non-renewable primary energy
excluding non-renewable primary energy resources used as raw materials; PENRM = Use of non-renewable primary energy resources used as raw
materials; PENRT = Total use of non-renewable primary energy resources; SM = Use of secondary material; RSF = Use of renewable secondary fuels;
NRSF = Use of non-renewable secondary fuels; FW = Use of net fresh water
RESULTS OF THE LCA – WASTE CATEGORIES AND OUTPUT FLOWS according to EN 15804+A2:
1 piece washbasin
Parameter Unit A1-A3 A4 A5 B1 B2 B3 B4 B5 B6 B7 C1 C2 C3 C4 D
HWD kg 1.78E-05 5.88E-11 8.3E-08 0 8.53E-03 0 0 0 0 0 0 6.04E-12 -2.29E-10 7.28E-11 -5.43E-11
NHWD kg 3.9E+00 2.59E-03 1.48E-01 0 8.92E-01 0 0 0 0 0 0 2.97E-04 2.33E-03 1.44E+01 -5.02E-04
6 Environmental Product Declaration - Hansgrohe Group - Washbasins
RWD kg 2.12E-03 3.2E-05 6.07E-04 0 4.67E-03 0 0 0 0 0 0 3.65E-06 4.73E-04 3.41E-05 -7.84E-05
CRU kg 0 0 0 0 0 0 0 0 0 0 0 0 0 0 0
MFR kg 0 0 1.12E+00 0 0 0 0 0 0 0 0 0 1.35E-01 0 0
MER kg 0 0 0 0 0 0 0 0 0 0 0 0 0 0 0
EEE MJ 0 0 4.09E-02 0 2.2E-01 0 0 0 0 0 0 0 0 0 0
EET MJ 0 0 7.27E-02 0 3.99E-01 0 0 0 0 0 0 0 0 0 0
HWD = Hazardous waste disposed; NHWD = Non-hazardous waste disposed; RWD = Radioactive waste disposed; CRU = Components for re-use;
MFR = Materials for recycling; MER = Materials for energy recovery; EEE = Exported electrical energy; EET = Exported thermal energy
RESULTS OF THE LCA – additional impact categories according to EN 15804+A2-optional:
1 piece washbasin
Parameter Unit A1-A3 A4 A5 B1 B2 B3 B4 B5 B6 B7 C1 C2 C3 C4 D
Disease
PM 1.26E-06 2.29E-07 3.1E-08 0 3.34E-06 0 0 0 0 0 0 3.48E-09 3.83E-09 1.9E-08 -5.84E-10
incidence
kBq U235
IR 4.53E-01 4.74E-03 9.42E-02 0 2.23E+00 0 0 0 0 0 0 5.44E-04 7.87E-02 3.98E-03 -1.3E-02
eq
ETP-fw CTUe 7.35E+011.34E+013.89E+00 0 1.73E+02 0 0 0 0 0 0 1.39E+001.55E+001.64E+00-1.42E-01
HTP-c CTUh 5.91E-09 2.66E-10 3.48E-09 0 2.51E-08 0 0 0 0 0 0 2.82E-11 5.83E-11 2.45E-10 -1.13E-11
HTP-nc CTUh 2.21E-07 1.11E-08 3.57E-07 0 6.84E-07 0 0 0 0 0 0 1.26E-09 1.35E-09 2.57E-08 -2.77E-10
SQP SQP 1.08E+025.88E+002.05E+01 0 3.38E+02 0 0 0 0 0 0 8.12E-01 1.59E+00 7.04E-01 -1.94E-01
PM = Potential incidence of disease due to PM emissions; IR = Potential Human exposure efficiency relative to U235; ETP-fw = Potential comparative
Toxic Unit for ecosystems; HTP-c = Potential comparative Toxic Unit for humans (cancerogenic); HTP-nc = Potential comparative Toxic Unit for humans
(not cancerogenic); SQP = Potential soil quality index
Disclaimer 1 – for the indicator “Potential Human exposure efficiency relative to U235”. This impact category deals mainly with the
eventual impact of low-dose ionizing radiation on human health of the nuclear fuel cycle. It does not consider effects due to possible
nuclear accidents, occupational exposure or radioactive waste disposal in underground facilities. Potential ionizing radiation from the
soil, radon and from some construction materials is also not measured by this indicator.
Disclaimer 2 – for the indicators “abiotic depletion potential for non-fossil resources”, “abiotic depletion potential for fossil resources”,
“water (user) deprivation potential, deprivation-weighted water consumption”, “potential comparative toxic unit for ecosystems”,
“potential comparative toxic unit for humans – cancerogenic”, “Potential comparative toxic unit for humans - not cancerogenic”,
“potential soil quality index”. The results of this environmental impact indicator shall be used with care as the uncertainties on these
results are high as there is limited experience with the indicator.
6. LCA: Interpretation
The figure above shows the dominance analysis over the The datasets that have relatively high contributions to many
considered modules. It can be seen here that the production included indicators are the dataset used for the soap in for
phase (modules A1-A3) as well as the maintenance (module maintenance (module B2), as well as the energy inputs (gas
B2) dominate the LCA results over the life cycle. GWP-biogenic and electricity) for the production of the ceramic.
is negative in modules A1-A3 due to biogenic carbon stored in
the packaging (cardboard and paper). The biogenic carbon Variability
balance is offset with the treatment of the packaging in module
A5. Module B2 is the same for all products. The results in the other
7 Environmental Product Declaration - Hansgrohe Group - Washbasins
modules are mainly dependend on the weight of the products impacts during production (A1-A3) and end-of-life (C-modules)
and the production location. since more materials and energies are required.
The weight of the products (incl. packaging) varies between 5.4 Keeping product weight constant there still is variability which is
and 35.7 kg (ceramic mass between 4.7 and 32.6 kg). In due to different production conditions of the two sites and
general, heavier products have higher potential environmental associated energy mixes.
7. Requisite evidence
8 Environmental Product Declaration - Hansgrohe Group - Washbasins
8. References
Standards (Federal Law Gazette 2833)
EN 13501-1
EN 13501-1:2019-05, Fire classification of construction CPR
products and building elements - Part 1: Classification using Construction Products Regulation
data from reaction to fire tests
Candidate list
Candidate List of substances of very high concern for
EN 14688 Authorisation, published in accordance with Article 59(10) of the
EN 14688:2018-12, Sanitary appliances - Wash basins - REACH Regulation. Helsinki: European Chemicals Agency
Functional requirements and test methods
IBU 2021
Institut Bauen und Umwelt e.V.: General Instructions for the
EN 15804 EPD programme of Institut Bauen und Umwelt e.V., Version
EN 15804:2012+A2:2019 + AC:2021, Sustainability of 2.0, Berlin: Institut Bauen und Umwelt e.V., 2021 www.ibu-
construction works — Environmental Product Declarations — epd.com
Core rules for the product category of construction products.
Managed LCA Content
Managed LCA Content. Content Version 2023.2. Leinfeld-
ISO 9001 Echterdingen: Sphera Solutions GmbH.
ISO 9001:2015-11, Quality management systems -
Requirements PCR part A
Product Category Rules for Building-Related Products and
Services. Part A: Calculation Rules for the Life Cycle
ISO 14025 Assessment and Requirements on the Project Report, Version
ISO 14025:2006-07, Environmental labels and declarations - 1.3. Berlin: Institut Bauen und Umwelt e.V. (ed.), 2021.
Type III environmental declarations - Principles and procedures
Further references
PCR: Sanitary ceramics
PCR Guidance-Texts for Building-Related Products and
AVV Services. Part B: Requirements on the EPDs for Sanitary
Waste Catalogue Ordinance (Abfallverzeichnis-Verordnung - Ceramics, Version 4. Berlin: Institut Bauen und Umwelt e.V.
AVV) of 10 December 2001 (Federal Law Gazette I p. 3379), (publisher.), 19.10.2023.
last amended by Article 2 of the Ordinance of 24 July 2002
9 Environmental Product Declaration - Hansgrohe Group - Washbasins
Publisher
Institut Bauen und Umwelt e.V. +49 (0)30 3087748- 0
Hegelplatz 1 info@ibu-epd.com
10117 Berlin www.ibu-epd.com
Germany
Programme holder
Institut Bauen und Umwelt e.V. +49 (0)30 3087748- 0
Hegelplatz 1 info@ibu-epd.com
10117 Berlin www.ibu-epd.com
Germany
Author of the Life Cycle Assessment
brands & values GmbH +49 421 70 90 84 33
Hollerallee 14A info@brandsandvalues.com
28209 Bremen www.brandsandvalues.com
Germany
Owner of the Declaration
Hansgrohe Group +49 7836 51-0
Auestr. 5-9 info@hansgrohe-group.com
77761 Schiltach www.hansgrohe-group.com
Germany
10 Environmental Product Declaration - Hansgrohe Group - Washbasins
