ENVIRONMENTAL PRODUCT DECLARATION
as per ISO 14025 and EN 15804+A2
Owner of the Declaration Unilin BV, division flooring
Publisher Institut Bauen und Umwelt e.V. (IBU)
Programme holder Institut Bauen und Umwelt e.V. (IBU)
Declaration number EPD-UNI-20230480-IBC1-EN
Issue date 15.01.2024
Valid to 14.01.2029
Direct Pressure Laminate floor coverings
Unilin BV, division flooring
www.ibu-epd.com | https://epd-online.com
1. General Information
Unilin BV, division flooring Direct Pressure Laminate floor coverings
Programme holder Owner of the declaration
IBU – Institut Bauen und Umwelt e.V. Unilin BV, division flooring
Hegelplatz 1 Ooigemstraat 3
10117 Berlin 8710 Wielsbeke
Germany Belgium
Declaration number Declared product / declared unit
EPD-UNI-20230480-IBC1-EN 1 m² of direct pressure laminate (DPL) floor covering of 7 mm thickness .
This declaration is based on the product category rules: Scope:
Floor coverings, 01.08.2021 The laminate floor covering described in this EPD has a thickness between
(PCR checked and approved by the SVR) 7 mm and 12 mm and meets the requirements of the EN14041:2006 and
the use classes between 31 and 34 according to EN 13329 and EN ISO
10874.
Issue date
The results are representative of production in UNILIN B.V. Division
15.01.2024
Flooring, Wielsbeke and Vielsalm sites (Belgium).
The products are available under following brandnames: Unilin, Quick-
Valid to
Step, Pergo, IVC Commercial, Sens by Quick-Step, Vitality, LocFloor,
14.01.2029 Clixfloor, PergoPro, Xpert Pro, Next, Easylife by Unilin, Lamidecor by
Unilin, Topfloor by Unilin, Expert click by Unilin, Artens by Unilin,
Goodhome, Piubell'arte, Les indispensables.
The owner of the declaration shall be liable for the underlying information
and evidence; the IBU shall not be liable with respect to manufacturer
information, life cycle assessment data and evidences.
The EPD was created according to the specifications of EN 15804+A2. In
the following, the standard will be simplified as EN 15804.
Verification
The standard EN 15804 serves as the core PCR
Dipl.-Ing. Hans Peters
Independent verification of the declaration and data according to ISO
(Chairman of Institut Bauen und Umwelt e.V.)
14025:2011
internally X externally
Florian Pronold Dr. Frank Werner,
(Managing Director Institut Bauen und Umwelt e.V.) (Independent verifier)
1 Environmental Product Declaration - Unilin BV, division flooring - Direct Pressure Laminate floor coverings
2. Product
• 1380mm x 156mm x 8mm
2.1 Product description/Product definition • 1380mm x 190mm x 8mm
DPL (Direct Pressure Laminate) floor coverings described in • 1380mm x 190mm x 8mm
this EPD are produced by UNILIN BV, division Flooring. The • 1380mm x 190mm x 12 mm
floor coverings meet the requirements of EN 13329. DPL • 1380mm x 212mm x 9mm
laminate floorings are made up of a number of layers. On the • 1380mm x 278,5mm x 8mm
top side, there is a decor with a transparent, wear-resistant • 2050mm x 205mm x 9,5mm
contact surface; in the middle, there is a core layer made of • 2050mm x 240mm x 9,5mm
high density wood fibre and on the back side, there is a • 1380mm x 190mm x 9mm
stabilizing layer to guarantee floor stability. The decorative
paper of DPL floor covering can be printed with any design and 2.5 Base materials/Ancillary materials
gives the floor its individual appearance. The planks have a The composition of a DPL floor covering in mass % is:
mechanical and patented connection (Uniclic, PerfectFold,
• 90-96 % High Density Wood Fibre board (HDF)
Aquafit, Unifit, Unidrop or Multifit).
• 2-4 % paper
• 4-6 % resin
For the placing on the market of the product in the European
• <1 % corundum
Union/European Free Trade Association (EU/EFTA) (with the
HDF (high density wood fibreboard)
exception of Switzerland) Regulation (EU) No. 305/2011 (CPR)
The core board is an HDF board >850kg/m³ composed of wood
applies. The product needs a declaration of performance taking
fibers and a thermosetting resin, mainly MUF (melamine-urea-
into consideration EN14041:2004 AC 2006 Resilient, textile and
formaldehyde) resin.
laminate floor coverings - Essential characteristics and the CE-
marking.
Paper
The renewable resource wood is the main raw material for
2.2 Application
paper production.
The laminate floor covering as described in this EPD is used as
a floating modular flooring system for indoor use and meets the
Resins
requirements of the use classes: between 31 and 34 according
The used amino resins are melamine-formaldehyde (95%) and
to EN 13329 and EN ISO 10874.
urea formaldehyde (5%) resins. Amino resins are thermosetting
2.3 Technical Data resins that are cured using heat and pressure.
The technical specifications of the products within the scope of
Corundum
the EPD shall be listed, including the reference to the test
Bauxite is the mineral resource of corundum. By using
methods/test standards for each specification.
aluminium oxide (Al2O3) the surface layer of a laminate flooring
obtains abrasion and scratch resistance.
For products with CE marking, the technical specifications must
be specified in accordance with information in the declaration of
This product contains substances listed in the Candidate List of
performance. The properties relevant to the product should be
Substances of Very High Concern for Authorisation REACH
specified in the table below. If no information is given for
(date: 16.11.2023) exceeding 0.1 percentage by mass: NO
properties, an explanation must be given in the background
report to the EPD as to why the property is not relevant to the
This product contains other CMR substances in categories 1A
product.
or 1B which are not on the candidate list, exceeding 0.1
percentage by mass: NO
Constructional data
Name Value Unit Biocide products were added to this construction product or it
Product minimum thickness 7 mm has been treated with biocide products (this then concerns a
Product maximum thickness 12 mm treated product as defined by the (EU) Ordinance on Biocide
Products No. 528/2012): NO
Product minimum mass (7 mm thickness) 6.4 kg/m²
Product maximum mass (12 mm thickness) 11.0 kg/m² 2.6 Manufacture
Abrasion Class AC4-AC6 - Impregnation & Resin production:
Product Form panel - The resin production is included in the LCA; it is produced by
UNILIN bvba, division Flooring. The different components are
Density 910 kg/m3
mixed together and used to impregnate the different paper
• Performance data of the product in accordance with the layers (overlay, décor and backing).
declaration of performance with respect to its essential
characteristics according to EN 14041:2004 AC 2006 Pressing:
Resilient, textile and laminate floor coverings - Essential The resin impregnated papers (overlay, décor and backing) are
characteristics. pressed under heat with the HDF core board in a single stage
process. In this process the resin cures and the different layers
2.4 Delivery status
are laminated together. The surface structure, the final gloss
Typical standard dimensions are as follows (length - width - and the bevelled edges for some products are applied during
thickness): the pressing phase.
• 1200mm x 190mm x 7mm
• 1200mm x 190mm x 8mm Cutting and milling:
• 1200mm x 396mm x 8mm The pressed boards are cut to size and equipped with a tongue
• 1224mm x 408mm x 8mm and-groove assembly system. Eventually the boards are
provided with a bevelled edge.
2 Environmental Product Declaration - Unilin BV, division flooring - Direct Pressure Laminate floor coverings
floor covering, the manufacturer's instructions concerning
Packaging: warranty and care must be observed, available for download at
The laminate floorings are unit-packed and edge-protected www.unilin.com/en/flooring. The use stage is declared in this
using cardboard boxes (5 sided) and shrink-wrapped in foil. EPD for a one year usage.
Laminate floor coverings are intended for use as floor covering Influences on ageing when applied in accordance with the rules
within a building. According to the area of application floor of technology.
coverings are classified in use classes.
2.13 Extraordinary effects
2.7 Environment and health during manufacturing Fire
The production conditions do not demand any special health The reaction to fire is determined according to EN 13501-1. The
protection measures over and beyond the legal requirements. class for laminate floors produced by UNILIN bvba-division
Flooring, in combination with all underlays of the sales program
Water is Cfl-s1. The classes 33 and 34 in the range are usually Bfl-
Production related waste water from the HDF production s1.
process is purified in a wastewater treatment plant. The use of
Fire protection
water in the DPL flooring production process is negligible.
Name Value
Where water is needed, it either evaporates or is re-used in the
internal water loop. Building material class Cfl or Bfl
Air Smoke gas development s1
The constitutional valid regulations are observed. The
emissions to air are far below the legally required thresholds.
Water
Soil
In case of a leak or a flood where the flooring has been soaked
There is no impact on soil.
for a longer period of time (days) the flooring will most probably
2.8 Product processing/Installation be considered a total loss. In case of short or shorter time of
exposure and after drying, no visible damage may be expected.
UNILIN Laminate floor coverings are generally installed floating.
If the water came under the floorcovering (floating installation) it
This means that the floor covering is not fixed to the sub-floor
may be necessary to un-click the planks/tiles and let them dry.
using glue, nails etc. The floor covering panels are mainly
The subfloor will most probably also be wet and should be
mechanically assembled glue-less by means of tongue and
given the time to come to equilibrium moisture content before
groove. Underlay material is needed when installing laminate
re-installation of the dry panels. Most of the laminate ranges
floor coverings in order to achieve a levelling effect, thermal or
offer a special water resistance and a watertight connection
acoustical insulation and/or protection against rising dampness.
between planks/tiles. During the installation, the periphery
2.9 Packaging needs to be treated with a foam strip and a special sealant to
Packaging requirements according to EN 13329: Laminate floor avoid infiltration. In case of water spillage on the surface, it will
coverings are delivered in packages designed to protect the evaporate before having the chance to penetrate between
corners, edges and surfaces of the product, under normal planks/tiles.
conditions of transport and handling. Laminate flooring is
accordingly unit-packed and edge-protected using ribbed Mechanical destruction
cardboard and shrinkwrapped in foil. Pallets are finally used for Small damages in the flooring surface can be repaired by using
the delivery. The pallets can also be reused. colored solvent-free melt waxes. In case of more severe
damage the damaged panels can be replaced. Procedures to
2.10 Condition of use repair or replace a damaged plank are available on request.
A thermosetting binding agent and saturating resin are used for The damaged panels go into the normal end-of-life treatment.
the production of the flooring panels. When heat and pressure
2.14 Re-use phase
are applied during the pressing phase, this is 3D crosslinked by
an irreversible polycondensation reaction. Under normal A laminate floor covering which is not at the end-of-life stage
conditions, the binding agent and saturating resin are both may be uninstalled and re-used as a floor covering. Post-
chemically stable and mechanically firmly bonded to the wood consumer laminate floor covering waste can be recycled as
parts. wood based products. When appropriate recycling facilities do
not exist, laminate floor coverings shall be thermally valorized.
2.11 Environment and health during use
2.15 Disposal
Environmental protection
When the products are used as designated and according the Post-installation and post-consumer flooring panels are
current state of knowledge, there are no hazards for water, air considered as wood waste. The European Waste Code EWC is
and soil. 030105. It can be disposed in any regulated municipal waste
collection point as wood waste.Unilin offers a take-back
Health protection program named Recover to enable circularity of Laminate
When used normally and in accordance with the designated flooring. Please contact your local Unilin dealer to check the
purpose, no health risks or restrictions are to be anticipated by availability of this Recover program in your country.
UNILIN DPL floor coverings. This is in line with the current state
2.16 Further information
of knowledge.
All information about the product composition, technical
2.12 Reference service life performance, instructions for installation and maintenance,
The BBSR Table gives a general useful life of 20 years for floor precautionary instructions for use, CE marking and relevant
coverings of component group 352.711. Due to the DOP (declaration of performance) documents, are available
comparatively high resistance of the laminate floorings, Unilin either in the packs or can be found on the homepage
grants an additional warranty (based on the floor owner life www.unilin.com/en/flooring or can be requested at Unilin BV
according to the manufacturer's warranty conditions) for the division flooring with the following address info@unilin.com.
declared product. In order to increase the life duration of the
3 Environmental Product Declaration - Unilin BV, division flooring - Direct Pressure Laminate floor coverings
3. LCA: Calculation rules
3.1 Declared Unit 3.4 Cut-off criteria
The declared unit is 1 m² laminate flooring with a thickness of 7 In the assessment, all available data from the production
mm and a weight of 6.4 kg. It has the use class 32 as this is the process are considered, i.e. all raw materials used, utilised
most common product. thermal energy, and electric power consumption using best
available LCI datasets. Thus material and energy flows
Declared unit and mass reference
contributing less than 1% of mass or energy are also
Name Value Unit
considered.
Declared unit 1 m2
Grammage 6.46 kg/m2 No flows were cut-off that are known to have significant
environmental impacts.
Layer thickness 0.007 m
3.5 Background data
3.2 System boundary
Used background data comes from ecoinvent database version
Type of EPD according to EN 15804: cradle to grave. 3.8 from 2021. It has been selected to be representative of
processes geographic location.
The production stage (A1-A3) includes all relevant processes
from "cradle-to-factory gate" within the cutoff rules. This 3.6 Data quality
includes for example the extraction and manufacture of all raw Primary data refer to the year 2021. The data of the foreground
materials and their delivery to the production site. processes is based on input-output analyses at the Belgian
The constructional process stage includes the delivery of the production sites. The primary data collection was done
floor covering to the point of installation (A4). A4 data are based thoroughly, all relevant flows were considered.
on a weighted average distance for worldwide deliveries.
3.7 Period under review
Installation stage (A5) is declared, accounting for electricity The period under review for primary data is 2021.
consumption, product installation losses, and packaging waste.
3.8 Geographic Representativeness
The use stage (B2) includes the cleaning of the laminate floor Land or region, in which the declared product system is
covering for 1 year. The cleaning frequencies are described in manufactured, used or handled at the end of the product´s
chapter 4. Provision of water, cleaning agent and electricity for lifespan: Global
the cleaning of the floor covering is considered.
3.9 Allocation
Product end-of-life (C1-C3) comprises the product dismantling,
The overall production of UNILIN comprises further products
transportation, and energy recovery in combined heat and
beside the product considered in this study. Data for thermal
power (CHP) plant. In module C3 the release of biogenic CO2
and electrical energy as well as auxiliary material refer to the
is declared according to EN 16485.
declared product. During data collection the allocation is done
via mass (kg). Specific information on allocation within the
Module D includes benefits from all net flows in the end-of-life
background data is given in the ecoinvent documentation.
stage that leave the product boundary system after having
passed the end-of-waste state. It is assumed that post- 3.10 Comparability
consumer flooring waste is incinerated as waste in a combined
Basically, a comparison or an evaluation of EPD data is only
heat and power (CHP) plant. Loads from material incineration
possible if all the data sets to be compared were created
and resulted benefits from recovered energy are declared
according to EN 15804 and the building context, respectively
within module D.
the product-specific characteristics of performance, are taken
into account.
3.3 Estimates and assumptions
Background database is as described in chapter 3.5.
No additional estimates or assumptions had to be made
beyond the information stated in clauses 3 and 4.
4. LCA: Scenarios and additional technical information
Transport to the construction site (A4)
Characteristic product properties of biogenic carbon
Product shipping stage A4 represents weighted average based
Information on describing the biogenic carbon content at on worldwide sales.
factory gate
Name ValueUnit
Name ValueUnit
Transport distance by truck 724 km
kg
Biogenic carbon content in product 2.49 Transport distance by boat 3029 km
C
Capacity utilisation (including empty runs) for truck 67 %
Biogenic carbon content in accompanying kg
0.109
packaging C Installation in the building (A5)
Note: 1 kg of biogenic carbon is equivalent to 44/12 kg of CO 2. Name Value Unit
Electricity consumption 0.04 kWh
Product installation losses 4.0 %
The following technical information is a basis for the declared
Product packaging waste 0.23 kg
modules. Scenarios correspond to the worldwide production
and consumption.
4 Environmental Product Declaration - Unilin BV, division flooring - Direct Pressure Laminate floor coverings
Maintenance (B2) End of Life (C1-C4)
Maintenance scenario is: Name Value Unit
• 1 vacuum cleaning per week, Collected separately waste type (wood waste) 6.46 kg
• 1 wet cleaning (water and detergent) per month. Energy recovery from waste 6.46 kg
Name Value Unit
100% of floor covering is incinerated in a combined heat and
Water consumption 1.33 kg/m²/year power (CHP) plant.
Detergent 0.0133 kg/m²/year
Electricity consumption (European mix) 0.54 kWh/m²/year Benefits and loads beyond the product system (D)
As per IBU PCR Part A, recovered heat is assumed to
substitute to heat generation from natural gas furnace for the
calculation of benefits and loads beyond the product system
Reference service life (module D). Produced electricity is assumed to substitute to
Name Value Unit grid mix.
Reference service life according to BBSR 20 a
5 Environmental Product Declaration - Unilin BV, division flooring - Direct Pressure Laminate floor coverings
5. LCA: Results
The results refer to the thickness of 7 mm (6.46 kg/m²) with use class 32. The information on maintenance is declared per year.
DPL laminate floor coverings are available in different thicknesses. In order to enable the user of the EPD to calculate the results for
different thicknesses and use classes the factors in the following table can be used for the calculation. For A1-A3, A4, A5, B2, C3 and D
the LCA results of the declared product (thickness 7 mm) in following tables have to be multiplied with these factors.
Extrapolation table - 8 mm thickness laminate floor covering
6 Environmental Product Declaration - Unilin BV, division flooring - Direct Pressure Laminate floor coverings
Extrapolation table - 9 mm thickness laminate floor covering
7 Environmental Product Declaration - Unilin BV, division flooring - Direct Pressure Laminate floor coverings
Extrapolation table - 9.5 mm thickness laminate floor covering
8 Environmental Product Declaration - Unilin BV, division flooring - Direct Pressure Laminate floor coverings
Extrapolation table - 12 mm thickness laminate floor covering
9 Environmental Product Declaration - Unilin BV, division flooring - Direct Pressure Laminate floor coverings
DESCRIPTION OF THE SYSTEM BOUNDARY (X = INCLUDED IN LCA; MND = MODULE OR INDICATOR NOT DECLARED; MNR
= MODULE NOT RELEVANT)
Benefits and
Construction loads beyond
Product stage Use stage End of life stage
process stage the system
boundaries
la ire ta m w a Ry lp p u s tro p s n a rT g n iru tc a fu n a M e h t m o rf tro p s n a rTe tis e h t o t e ta g y lb m e s s A e s U e c n a n e tn ia M ria p e R tn e m e c a lp e R tn e m h s ib ru fe R y g re n e la n o ita re p Oe s u re ta w la n o ita re p Oe s u n o itc u rts n o c -e Dn o itilo m e d tro p s n a rT g n is s e c o rp e ts a W la s o p s iD -e s u e R-y re v o c e R-g n ilc y c e Rla itn e to p
A1 A2 A3 A4 A5 B1 B2 B3 B4 B5 B6 B7 C1 C2 C3 C4 D
X X X X X MND X MNR MNR MNR MND MND X X X X X
RESULTS OF THE LCA - ENVIRONMENTAL IMPACT according to EN 15804+A2: 1 m² direct pressure laminate floor covering
Parameter Unit A1 A2 A3 A4 A5 B2 C1 C2 C3 C4 D
GWP-total kg CO 2 eq -4.42E+00 1.51E-01 9.75E-01 9.74E-01 7.67E-01 2.29E-01 0 4.46E-02 9.26E+00 0 -7.3E+00
GWP-fossil kg CO 2 eq 4.51E+00 1.51E-01 1.25E+00 9.73E-01 3.71E-01 2.25E-01 0 4.45E-02 1.44E-01 0 -7.29E+00
GWP-
biogenic kg CO 2 eq -8.94E+00 4.87E-05 -2.82E-01 2.86E-04 3.96E-01 1.19E-03 0 1.45E-05 9.12E+00 0 -5.95E-03
GWP-luluc kg CO 2 eq 1.01E-02 5.91E-05 2.8E-03 4.59E-04 5.71E-04 2.89E-03 0 1.72E-05 6.89E-05 0 -2.71E-03
kg CFC11
ODP 1.23E-05 3.78E-08 1.73E-06 2.21E-07 5.73E-07 1.63E-08 0 1.12E-08 4.93E-09 0 -1E-06
eq
AP mol H+ eq 3.28E-02 5.29E-04 7.74E-03 8.45E-03 2.22E-03 1.29E-03 0 1.43E-04 8.8E-03 0 -1.1E-02
EP-
kg P eq 1.91E-04 1.08E-06 4.49E-05 6.32E-06 1.33E-05 2.47E-05 0 3.2E-07 1.81E-05 0 -1.19E-04
freshwater
EP-marine kg N eq 7.87E-03 1.17E-04 2.23E-03 1.97E-03 5.77E-04 2.08E-04 0 3.15E-05 3.88E-03 0 -2.22E-03
EP-terrestrial mol N eq 9.87E-02 1.3E-03 2.56E-02 2.19E-02 6.91E-03 1.95E-03 0 3.5E-04 4.57E-02 0 -2.47E-02
kg NMVOC
POCP 2.65E-02 4.95E-04 7.15E-03 6.3E-03 1.88E-03 5.35E-04 0 1.38E-04 1.05E-02 0 -7.98E-03
eq
ADPE kg Sb eq 5.57E-05 3.74E-07 1.02E-05 3.14E-06 3.01E-06 2.24E-06 0 1.11E-07 2.36E-06 0 -3.55E-06
ADPF MJ 9.34E+01 2.46E+00 3.48E+01 1.44E+01 6.14E+00 4.78E+00 0 7.31E-01 2.31E+00 0 -1.31E+02
m3 world eq
WDP 5.57E+00 8.44E-03 1.05E+00 4.07E-02 2.74E-01 6.49E-02 0 2.51E-03 3.7E-02 0 -2.88E-01
deprived
GWP = Global warming potential; ODP = Depletion potential of the stratospheric ozone layer; AP = Acidification potential of land and water; EP =
Eutrophication potential; POCP = Formation potential of tropospheric ozone photochemical oxidants; ADPE = Abiotic depletion potential for non-fossil
resources; ADPF = Abiotic depletion potential for fossil resources; WDP = Water (user) deprivation potential)
RESULTS OF THE LCA - INDICATORS TO DESCRIBE RESOURCE USE according to EN 15804+A2: 1 m² direct pressure
laminate floor covering
Parameter Unit A1 A2 A3 A4 A5 B2 C1 C2 C3 C4 D
PERE MJ 2.8E+01 3.12E-02 2.81E+01 1.88E-01 8.31E+00 9.84E-01 0 9.3E-03 9.56E+01 0 -4.38E+00
PERM MJ 9.44E+01 0 1.92E+00 0 -2.11E+00 8.77E-04 0 0 -9.39E+01 0 0
PERT MJ 1.22E+02 3.12E-02 3E+01 1.88E-01 6.21E+00 9.85E-01 0 9.3E-03 1.67E+00 0 -4.38E+00
PENRE MJ 7.57E+01 2.46E+00 3.4E+01 1.44E+01 6.99E+00 4.42E+00 0 7.31E-01 1.98E+01 0 -1.31E+02
PENRM MJ 1.77E+01 0 7.87E-01 0 -8.54E-01 3.64E-01 0 0 -1.75E+01 0 0
PENRT MJ 9.34E+01 2.46E+00 3.48E+01 1.44E+01 6.14E+00 4.78E+00 0 7.31E-01 2.31E+00 0 -1.31E+02
SM kg 1.77E-03 0 7.86E-02 0 3.21E-03 3.28E-04 0 0 0 0 0
RSF MJ 0 0 0 0 0 0 0 0 0 0 0
NRSF MJ 0 0 0 0 0 0 0 0 0 0 0
FW m3 1.46E-01 2.86E-04 2.79E-02 1.46E-03 7.5E-03 4.2E-03 0 8.51E-05 6.12E-03 0 -2.06E-02
PERE = Use of renewable primary energy excluding renewable primary energy resources used as raw materials; PERM = Use of renewable primary
energy resources used as raw materials; PERT = Total use of renewable primary energy resources; PENRE = Use of non-renewable primary energy
excluding non-renewable primary energy resources used as raw materials; PENRM = Use of non-renewable primary energy resources used as raw
materials; PENRT = Total use of non-renewable primary energy resources; SM = Use of secondary material; RSF = Use of renewable secondary fuels;
NRSF = Use of non-renewable secondary fuels; FW = Use of net fresh water
RESULTS OF THE LCA – WASTE CATEGORIES AND OUTPUT FLOWS according to EN 15804+A2:
1 m² direct pressure laminate floor covering
Parameter Unit A1 A2 A3 A4 A5 B2 C1 C2 C3 C4 D
HWD kg 1.9E-01 1.72E-03 5.99E-02 1.12E-02 1.73E-02 5.89E-03 0 5.06E-04 4.51E-02 0 -3.32E-02
NHWD kg 3.35E+00 2.41E-01 6.85E-01 7.13E-01 2.15E-01 8.9E-02 0 7.21E-02 1.12E-01 0 -3.81E-01
RWD kg 4.1E-04 1.67E-05 2.3E-04 9.79E-05 3.07E-05 3.39E-05 0 4.95E-06 2.44E-05 0 -2.31E-04
CRU kg 0 0 0 0 0 0 0 0 0 0 0
MFR kg 1.37E-03 0 1.7E-02 0 7.36E-04 4.25E-04 0 0 0 0 0
MER kg 0 0 0 0 0 0 0 0 0 0 0
EEE MJ 3.6E-01 0 1.82E+00 0 1.09E+00 1.48E-03 0 0 9.29E+00 0 0
EET MJ 6.95E-01 0 3.5E+00 0 2.11E+00 2.86E-03 0 0 8.91E+01 0 0
10 Environmental Product Declaration - Unilin BV, division flooring - Direct Pressure Laminate floor coverings
HWD = Hazardous waste disposed; NHWD = Non-hazardous waste disposed; RWD = Radioactive waste disposed; CRU = Components for re-use;
MFR = Materials for recycling; MER = Materials for energy recovery; EEE = Exported electrical energy; EET = Exported thermal energy
RESULTS OF THE LCA – additional impact categories according to EN 15804+A2-optional:
1 m² direct pressure laminate floor covering
Parameter Unit A1 A2 A3 A4 A5 B2 C1 C2 C3 C4 D
Disease
PM 9.26E-07 1.74E-08 1.82E-07 6.94E-08 4.98E-08 4.19E-09 0 5.2E-09 1.72E-07 0 -3.34E-08
incidence
IR kBq U235 eq 3.29E-01 1.07E-02 2.51E-01 6.25E-02 2.66E-02 4.1E-02 0 3.17E-03 4.56E-02 0 -2.43E-01
ETP-fw CTUe 2.7E+01 8.15E-01 5.83E+00 4.89E+00 1.85E+00 8.04E-01 0 2.42E-01 3.42E+00 0 -4.84E+00
HTP-c CTUh 2.47E-08 5.32E-11 4.15E-09 4.17E-10 1.32E-09 1.1E-10 0 1.56E-11 1.69E-09 0 -8.6E-10
HTP-nc CTUh 8.42E-08 1.67E-09 1.95E-08 8.35E-09 5.39E-09 2.98E-09 0 4.98E-10 4.8E-08 0 -1.24E-08
SQP SQP 5.24E+02 2.8E+00 1.11E+02 8.68E+00 2.6E+01 1.05E+00 0 8.36E-01 6.8E-01 0 -6.02E+00
PM = Potential incidence of disease due to PM emissions; IR = Potential Human exposure efficiency relative to U235; ETP-fw = Potential comparative
Toxic Unit for ecosystems; HTP-c = Potential comparative Toxic Unit for humans (cancerogenic); HTP-nc = Potential comparative Toxic Unit for humans
(not cancerogenic); SQP = Potential soil quality index
Disclaimer 1 – for the indicator “Potential Human exposure efficiency relative to U235”. This impact category deals mainly with the
eventual impact of low-dose ionizing radiation on human health of the nuclear fuel cycle. It does not consider effects due to possible
nuclear accidents, occupational exposure or radioactive waste disposal in underground facilities. Potential ionizing radiation from the
soil, radon and from some construction materials is also not measured by this indicator.
Disclaimer 2 – for the indicators “abiotic depletion potential for non-fossil resources”, “abiotic depletion potential for fossil resources”,
“water (user) deprivation potential, deprivation-weighted water consumption”, “potential comparative toxic unit for ecosystems”,
“potential comparative toxic unit for humans – cancerogenic”, “Potential comparative toxic unit for humans - not cancerogenic”,
“potential soil quality index”. The results of this environmental impact indicator shall be used with care as the uncertainties on these
results are high as there is limited experience with the indicator.
6. LCA: Interpretation
Benefits and burdens beyond the system boundary (module D)
vary from a few percent to about 100% (GWP - fossil) of the
impacts over the product life cycle (modules A-C) and relate
basically to the energy recovery from waste processing in a
combined heat and power plant that is considered to substitute
natural gas (heat) and electricity grid mix.
Figure : Indicator results of direct pressure laminate floor
covering over its life cycle
The largest part of environmental impacts is caused during
production (modules A1-A3) and at waste processing (module
C3); comparably small impacts are caused during the transport
of the product to the construction site.
Maintenance (module B2) is presented for 1 year of product
use, so its impact can be significant over the reference service
life depending on the considered indicator.
All the other modules related to the product life cycle are not
significant.
11 Environmental Product Declaration - Unilin BV, division flooring - Direct Pressure Laminate floor coverings
7. Requisite evidence
7.1 PEFC certificate by Servaco/Normec Product Testing - Honderweg 13 - 9230
The product fulfills the requirements according to PEFC ST Wetteren - Belgium. Emission test report of Unilin sample
2002: 2010: Chain of Custody of Forest Based Products - 'Unilin group laminate 12mm thickness' nr SPT2021-R190 from
Requirements, second edition. CTIB - TCHN- Hof ter Vleest November 8th 2021.
dreef 3 - 1070 Brussel - Belgium.
• Compliant with AgBB-Scheme 2018 and 2021
• Compliant with M1 Emission Classification of Building
7.2 CE marking
Materials Testing protocol 15.11.2017)
CE-labelling according to EN 14041, type 3 – notified body:
• Compliant with the French VOC-Regulation: A+
0380-1161.
VOC EMISSION RESULTS (AgBB) AFTER 3 DAYS
7.3 Formaldehyde emissions Name Value Unit
Determination of the formaldehyde emission of a 12mm TVOC 550 µg/m3
laminate flooring according to AgBB-Scheme, ISO 16000 part
R (dimensionless) 0,104
3, 6 and 9. by Servaco/Normec Product Testing - Honderweg
TVOC without LCI < 5 µg/m3
13 - 9230 Wetteren - Belgium. Emission test report of Unilin
sample 'Unilin group laminate 12mm thickness' nr SPT2021- Carcinogenous < 1 µg/m3
R190 from November 8th 2021. VOC EMISSION RESULTS (AgBB) AFTER 28 DAYS
Name Value Unit Name Value Unit
Formaldehyde CAS nr 50-00-0 79 µg/m3 TVOC 110 µg/m3
R (dimensionless) 0.245
7.4 VOC emissions
VOC without LCI 6 µg/m3
Determination of the VOC emissions of a 12mm laminate
flooring according to AgBB-Scheme, ISO 16000 part 3, 6 and 9. Carcinogens < 1 µg/m3
8. References
IBU 2021 volatile organic compounds in indoor and test chamber air by
Institut Bauen und Umwelt e.V.: General Instructions for the active sampling on Tenax A sorbent, thermal desorption an gas
EPD programme of Institut Bauen und Umwelt e.V., Version chromatography using MS of MS-FID
2.0, Berlin: Institut Bauen und Umwelt e.V., 2021 www.ibu-
epd.com ISO 16000-9:2006
ISO 16000-9:20006 – Indoor air – part 9: Determination of the
EN 15804 emissions of volatile organic compounds from building products
EN 15804:2012+A2:2019+AC:2021, Sustainability of and furnishing – Emission test chamber method.
construction works —
Environmental Product Declarations — Core rules for the EN ISO 10874:2012
product category EN ISO 10874:2012/A1:2021Resilient, textile and laminate floor
of construction products. coverings - Classification
EN ISO 14044 EN 14041:2004
Environmental management - Life cycle assessment - EN 14041:2004 AC 2006 – Resilient, textile, laminate and
Requirements and guidelines (ISO 14044:2006); German and modular multilayer floor coverings - Essential characteristics
English version EN ISO 14044 Resilient, textile and laminate floor coverings
ISO 14025 EN 13329:2016
EN ISO 14025:2011, Environmental labels and declarations — EN 13329:2016+A2:2021
Type III environmental declarations — Principles and Laminate floor coverings - Elements with a surface layer based
procedures. on aminoplastic thermosetting resins - Specifications,
requirements and test methods
ISO 14040
ISO 14040:2006, Environmental management - Life cycle prEN 13329:2023
assessment - Principles and framework (ISO 14040); German Laminate floor coverings - Specifications, requirements and test
and English version EN ISO 14040 methods
Bundesinsitut für Bau-, Stadt- und Raumforschung.
EN/TR 15941
Sustainability of construction works - Environmental product EWC-94/3/EC
declarations - Methodology for selection and use of generic Commission Decision of 20 December 1993 establishing a list
data; German version CEN/TR 15941 of wastes pursuant to Article 1a of Counsil Directive
ISO 16000-3:2011 74/442/EEC on waste, 1993 - European Waste Catalogue and
Hazardous Waste List valid from 1 January 2002.
ISO 16000-3:2011 – Indoor air – part3: Determination of
formaldehyde and other carbonyl compounds in indoor air and ecoinvent
test chamber air – Active sampling method. ecoinvent, Allocation, cut-off by classification, ecoinvent
database version 3.8 (2021)
ISO 16000-6:2011
ISO 16000-6:2011 – Indoor air – part 6: Determination of PCR Guidance – Texts for Building-Related Products and
12 Environmental Product Declaration - Unilin BV, division flooring - Direct Pressure Laminate floor coverings
Services – Part B: Requirements on the EPD for floor in the EPD do not need to be listed here again.
coverings - IBU Published v6 dated 19.10.2023 The current version of PCR Part A and PCR Part B of the PCR
The literature referred to in the Environmental Product document on which they are based must be referenced.
Declaration must be listed in full.Standards already fully quoted
13 Environmental Product Declaration - Unilin BV, division flooring - Direct Pressure Laminate floor coverings
Publisher
Institut Bauen und Umwelt e.V. +49 (0)30 3087748- 0
Hegelplatz 1 info@ibu-epd.com
10117 Berlin www.ibu-epd.com
Germany
Programme holder
Institut Bauen und Umwelt e.V. +49 (0)30 3087748- 0
Hegelplatz 1 info@ibu-epd.com
10117 Berlin www.ibu-epd.com
Germany
Author of the Life Cycle Assessment
EVEA +33 2 28 07 87 00
rue Arthur III, 11 contact@evea-conseil.com
44200 Nantes www.evea-conseil.com/en
France
Owner of the Declaration
Unilin BV, division flooring +32 56 67 52 11
Ooigemstraat 3 info@unilin.com
8710 Wielsbeke www.unilin.com/en/flooring
Belgium
14 Environmental Product Declaration - Unilin BV, division flooring - Direct Pressure Laminate floor coverings
