ENVIRONMENTAL PRODUCT DECLARATION
as per ISO 14025 and EN 15804+A1
Owner of the Declaration Stiferite
Publisher Institut Bauen und Umwelt e.V. (IBU)
Programme holder Institut Bauen und Umwelt e.V. (IBU)
Declaration number EPD-STF-20200243-CBA3-EN
Issue date 18.12.2020
Valid to 17.12.2025
Stiferite BB average thick panel
Stiferite
www.ibu-epd.com | https://epd-online.com
General Information
Stiferite Stiferite BB average thick panel
Programme holder Owner of the declaration
IBU – Institut Bauen und Umwelt e.V. Stiferite
Hegelplatz 1 Viale Navigazione Interna 54
10117 Berlin 35129 Padova
Germany Italy
Declaration number Declared product / declared unit
EPD-STF-20200243-CBA3-EN STIFERITE BB expanded rigid polyurethane foam , covered on both sides
by bituminous paper facers, and produced by Stiferite. The EPD applies to
1 m2 of an average 75 mm thick PIR sandwich board, i.e. 0.075 m3, with
an average density between foam and facing of 31.3 kg/m3.
This declaration is based on the product category rules: Scope:
Insulating materials made of foam plastics, 01.08.2021 Stiferite spa produces STIFERITE BB that is a high performance insulation
(PCR checked and approved by the SVR) board manufactured from closed cell expanded rigid polyurethane foam,
covered on both sides by bituminous paper facers.The data have been
provided by the only Stiferite factory that was located in Padova (Italy) for
Issue date the year 2019.The owner of the declaration shall be liable for the
underlying information and evidence; the IBU shall not be liable with
18.12.2020
respect to manufacturer information, life cycle assessment data and
evidences
The owner of the declaration shall be liable for the underlying information
Valid to
and evidence; the IBU shall not be liable with respect to manufacturer
17.12.2025 information, life cycle assessment data and evidences.
The EPD was created according to the specifications of EN 15804+A1. In
the following, the standard will be simplified as EN 15804.
Verification
The standard EN 15804 serves as the core PCR
Independent verification of the declaration and data according to ISO
14025:2011
internally X externally
Dipl.-Ing. Hans Peters
(Chairman of Institut Bauen und Umwelt e.V.)
Dipl.-Ing. Hans Peters Prof. Dr. Birgit Grahl,
(Managing Director Institut Bauen und Umwelt e.V.) (Independent verifier)
1 Environmental Product Declaration - Stiferite - Stiferite BB average thick panel
Product
This provides a thermal resistance R = 2.73 m² k/W.
Product description/Product definition
STIFERITE'S thermo insulation panels are mainly used in the
building/construction sector and that of industrial insulation.
The panels are made of thermo-setting closed cells Base materials/Ancillary materials
polyurethane foam (PU) supplied with various types of flexible Core material (about 78.8 % of the weight of the declared
facers on both sides of the panel. The nature/type of unit):
facercontributes to the performance characteristics of the Closed-cell Polyiso (PIR) rigid foam made from MDI (50-65 %),
product and its application. polyols (20-30 %), pentane (4-5 %) and additives (4-7 %).
Expanded rigid polyurethane foam is distinguished by its' Facing (about 26,1 % of the weight of the declared unit):
excellent thermo insulation performance, mechanical bituminous paper consisting of kraft paper (60-70%) and
resistance, workability, lightness, and durability. bitumen (40-30%).
The performance of STIFERITE'S panels is determined based
on the European norm EN 13165:2012+A2:2016 Thermal The PU board for insulation:
insulation products for buildings - Factory made rigid
• This product/article/at least one partial article contains
polyurethane foam (PU) products - Specification.
substances listed in the candidate list (date: 17.11.2020)
This EPD refers to STIFERITE BB Average thick panel, made
exceeding 0.1 percentage by mass: no
of an insulation component in polyurethane foam using blowing
• This product/article/at least one partial article doesn't
agent Pentane-based, covered on both sides by bituminous
contain other CMR substances in categories 1A or 1B
paper.
which are not on the candidate list, exceeding 0.1
The panel is produced in standard dimensions of 600 x 1200
percentage by mass: no
mm and straight finish borders. Upon request and for minimum
• Biocide products were added to this construction
quantities, the panels may be produced in various dimensions.
product or it has been treated with biocide products (this
STIFERITE BB Average thick panel is produced by a certified
then concerns a treated product as defined by the (EU)
company with systems: ISO 9001, ISO 45001, ISO 14001 in its
Ordinance on Biocide Products No. 528/2012): no
entire line of products. For the placing on the market of the
Additional declaration according to quoted law: The product is
product in the EuropeanUnion/European Free Trade
compliant with all requirements indicated at chapter 2.5.7
Association (EU/EFTA) (with the exception of Switzerland) the
'Isolanti termici ed acustici' of the n.256 D.L. of the 23th June
Regulation (EU) No. 305/2011 (CPR) applies. The product
2022 (CAM EDILIZIA):
needs a Declaration of Performance taking into consideration
• Any blowing agent with Ozone depletion potential >0 is
EN 13165:2012+A2:2016 Thermal insulation products for
not used in production
building- factory made rigid polyurethane foam (PU) products -
• Any substances of Very High Concern-SVHC in
Specification and the CE-marking. For the application and use
concentration of more than 0,1 %w are not used in
the respective national provisions apply.
production (REACH n. 1907/2006). Any specific
Application authorizations for use are eserved provided for by the
The STIFERITE BB panel is suited for walk-on roofs, paved same Regulation for the substances included in Annex
roofs and foor insulation. XIV and specifications restrictions set out in Annex XVII
of the Regulation.
Technical Data • Catalysts lead-based are not used in production
The data provided by the Declaration of Performance apply. In • Flame retardants used in production (belonging to the
this Life Cycle Assessment, a PU insulation board with the Organophosphorus class) are not banned by any
following properties has been regarded: national or European regulation
• According to the raw materials declarations of suppliers
Constructional data
the minimum amount of recycled raw materials based
Name Value Unit
on the insulation board (PU foam and facers) weight is 3
Gross density 31.3 kg/m3 %w and the minimum amount of recycled raw materials
Declared average Thermal conductivity λD acc. to based on the PU insulation foam weight is 4 %w (note:
0.027 W/mK
/EN 13165/ this information is not explicitly considered in the LCA
and not included in the EPD tables that only refer to
Compressive strength at 10% deformation acc. to
> 150 kPa recycling content in the foreground system).
/EN 826/
Tensile strength perpendicular to the face acc. to Reference service life
> 40 kPa
/EN 1607/
The durability of insulation panels is normally at least as long as
Water absorption by total immersion acc. to /EN Vol.- the lifetime of the building in which it is used. The experimental
< 5
12087/ % data show that the reference life is longer than 50 years, Clima
Water absorption by partial immersion acc. to /EN 2019 .
< 0.3 kg/m²
1609/
Water vapour diffusion resistance factor μ acc. to
87
/EN 12086/
Euroclass reaction to fire acc. to /EN 11925/ F
LCA: Calculation rules
The declared unit is 1 m² with an average thickness of 75 mm,
Declared Unit e. g. 0.075 m³. Corresponding conversion factors are listed in
the table below.
2 Environmental Product Declaration - Stiferite - Stiferite BB average thick panel
construction site, the installation and the end-of-life stage of the
Declared unit
used PU thermal insulation board. The life cycle is split into the
Name Value Unit
following individual phases:
Declared unit 1 m2 A1 - Raw material formulation
Gross density 31.3 kg/m3 A2 - Raw material transport
A3 - Production of the insulation board and packaging material
Volume 0.075 m³
A4 - Transport to the construction site
Grammage 235 kg/m2
A5 - Emissions and cutting losses during installation and
Declared average thermal conductivity λD 0.027 W/mK packaging disposal
Layer thickness 0.075 m C2 - Transport to end of life
Conversion factor to 1 kg 2.35 kg/m² C3/C4 - End-of-Life: waste management (thermal recovery,
landfill)
Weight of declared unit 2.35 kg/m²
D - Benefits and loads beyond system boundary
This provides a thermal resistance R = 2.73 m2K/W.
Geographic Representativeness
The LCI data used in this report refer to an average product Land or region, in which the declared product system is
having an average thickness (material in the repipes of different manufactured, used or handled at the end of the product´s
thicknesses are weighted according to the relative production in lifespan: Italy
square meters). The type of declaration is 1 c - declaration of
an average product from a manufacturer's plant.
Comparability
Basically, a comparison or an evaluation of EPD data is only
possible if all the data sets to be compared were created
System boundary according to EN 15804 and the building context, respectively
This life cycle assessment for the production of the the product-specific characteristics of performance, are taken
polyurethane insulation board considers the life cycle from the into account. For life
supply of raw materials to the manufacturer´s gate (cradle-to- cycle modelling of the considered products, the GaBi 9 2020
gate with options). It also includes the transport to the has been used.
LCA: Scenarios and additional technical information
Name Value Unit
The following technical scenario information is required for the
Material loss 0.0469 kg
declared modules and optional for non-declared modules.
VOC in the air Pentane 1.27E-06 kg
Modules for which no information is declared can be deleted;
additional information can also be listed if necessary.
End of life (C1-C4)
The following technical information is a basis for the declared
The results for the end-of-life are declared for the 2 different
modules or can be used for developing specific scenarios in the
scenarios:
context of a building assessment if modules are not declared
(MND). Name Value Unit
Scenario No 1: Material Incineration 100 %
A5 is not declared including the disposal of the packaging Scenario No 2: Landfill 100 %
material on the construction site, the amounts of packaging
C4: Disposal scenarios used is divided into the 2
materials included in the LCA calculations must be declared as
sub-scenarios:
technical scenario information for Module A5.
1) Incineration 100% (C4/1)
2) Landfilling 100% (C4/2)
Transport to the building site (A4)
D: Benefits and loads beyond system boundary is divided into
The distances calculated are weighted average distances the 2 sub-scenarios:
according to the overall sales distribution; such distribution is 1) Incineration 100% (D1)
considered similar for all Stiferite products. 2) Landfilling 100% (D2)
Name ValueUnit
Truck with a capacity of 17.3 tons 270 km Reuse, recovery and/or recycling potentials (D), relevant
Ferry with a capacity of 1200-10000 dwt payload scenario information
124 km
capacity Name Value Unit
Ship with a capacity of 27500 dwt payload capacity
11000 km Module D includes credits from recycling materials of insulation
tons
panels and packaging, energy credits from thermal recovery of
Plane with a capacity of 22 ton 0 km the packaging. The results are declared for the same 3 different
scenarios described above.
Installation into the building (A5)
3 Environmental Product Declaration - Stiferite - Stiferite BB average thick panel
LCA: Results
The tables below show the results of the LCA. Basic information on all declared modules provides chapter 4.
There are two scenarios for the end-of-life (C3, C4 and D) analyzed: Scenario 1 considers 100% incineration, Scenario 2 considers
100% landfill disposal.
For SM, RSF, NRSF,CRU indicators only the foreground system is considered.
DESCRIPTION OF THE SYSTEM BOUNDARY (X = INCLUDED IN LCA; MND = MODULE NOT DECLARED; MNR = MODULE NOT
RELEVANT)
Benefits and
Construction loads beyond
Product stage Use stage End-of-life stage
process stage the system
boundaries
la ire ta m w a Ry lp p u s tro p s n a rT g n iru tc a fu n a M e h t m o rf tro p s n a rTe tis e h t o t e ta g y lb m e s s A e s U e c n a n e tn ia M ria p e R tn e m e c a lp e R tn e m h s ib ru fe R y g re n e la n o ita re p Oe s u re ta w la n o ita re p Oe s u n o itc u rts n o c -e Dn o itilo m e d tro p s n a rT g n is s e c o rp e ts a W la s o p s iD -e s u e R-y re v o c e R-g n ilc y c e Rla itn e to p
A1 A2 A3 A4 A5 B1 B2 B3 B4 B5 B6 B7 C1 C2 C3 C4 D
X X X X X MND MND MNR MNR MNR MND MND MND X X X X
RESULTS OF THE LCA - ENVIRONMENTAL IMPACT according to EN 15804+A1: 1 m² BB insulation panel
Parameter Unit A1-A3 A4 A5 C2 C3/1 C3/2 C4/1 C4/2 D/1 D/2
GWP kg CO 2 eq 5.37E+00 4.44E-02 8.71E-01 1.1E-02 0 0 4.47E+00 3.58E+01 -2.01E+00 -1.46E+00
ODP kg CFC11 eq 8.34E-06 9.77E-18 1.67E-07 2.74E-18 0 0 2.63E-15 1.32E-14 -4.25E-14 -4.28E-14
AP kg SO 2 eq 1.21E-02 4.04E-04 5.27E-04 2.42E-05 0 0 1.88E-03 1.29E-02 -3.32E-03 -3.02E-03
EP kg PO 43 eq 2.38E-03 5.41E-05 1.34E-03 5.87E-06 0 0 4.53E-04 6.43E-02 -3.89E-04 -3.35E-04
POCP kg Ethen eq 1.03E-02 -7.64E-06 3.85E-04 -7.79E-06 0 0 1.2E-04 8.86E-03 -2.66E-04 -2.17E-04
ADPE kg Sb eq 1.12E-05 3.4E-09 2.44E-07 1.01E-09 0 0 1.13E-07 7.48E-07 -5.05E-07 -4.82E-07
ADPF MJ 1.3E+02 5.89E-01 3.78E+00 1.49E-01 0 0 2.04E+00 5.27E+01 -2.63E+01 -1.67E+01
GWP = Global warming potential; ODP = Depletion potential of the stratospheric ozone layer; AP = Acidification potential of land and water; EP =
Eutrophication potential; POCP = Formation potential of tropospheric ozone photochemical oxidants; ADPE = Abiotic depletion potential for non-fossil
resources; ADPF = Abiotic depletion potential for fossil resources
RESULTS OF THE LCA - INDICATORS TO DESCRIBE RESOURCE USE according to EN 15804+A1: 1 m² BB insulation panel
Parameter Unit A1-A3 A4 A5 C2 C3/1 C3/2 C4/1 C4/2 D/1 D/2
PERE MJ 2.34E+01 IND 6.11E-01 IND IND IND 6.48E-01 IND IND IND
PERM MJ 2.21E+00 IND 0 IND IND IND 0 IND IND IND
PERT MJ 2.56E+01 2.69E-02 6.11E-01 8.63E-03 0 0 6.48E-01 4.25E+00 -1.13E+01 -1.14E+01
PENRE MJ 6.18E+01 IND 2.95E+00 IND IND IND 7.68E+01 IND IND IND
PENRM MJ 7.6E+01 IND -1.72E+00 IND IND IND -7.43E+01 IND IND IND
PENRT MJ 1.38E+02 5.92E-01 1.22E+00 1.5E-01 0 0 2.54E+00 5.47E+01 -3.6E+01 -2.65E+01
SM kg 0 0 0 0 0 0 0 0 0 0
RSF MJ 0 0 0 0 0 0 0 0 0 0
NRSF MJ 0 0 0 0 0 0 0 0 0 0
FW m3 6.01E-02 3.16E-05 1.43E-03 1.01E-05 0 0 1.07E-02 5.49E-03 -1.31E-02 -1.32E-02
PERE = Use of renewable primary energy excluding renewable primary energy resources used as raw materials; PERM = Use of renewable primary
energy resources used as raw materials; PERT = Total use of renewable primary energy resources; PENRE = Use of non-renewable primary energy
excluding non-renewable primary energy resources used as raw materials; PENRM = Use of non-renewable primary energy resources used as raw
materials; PENRT = Total use of non-renewable primary energy resources; SM = Use of secondary material; RSF = Use of renewable secondary fuels;
NRSF = Use of non-renewable secondary fuels; FW = Use of net fresh water
RESULTS OF THE LCA – WASTE CATEGORIES AND OUTPUT FLOWS according to EN 15804+A1:
1 m² BB insulation panel
Parameter Unit A1-A3 A4 A5 C2 C3/1 C3/2 C4/1 C4/2 D/1 D/2
HWD kg 1.08E-05 2.13E-08 2.2E-07 6.93E-09 0 0 2.79E-09 2.01E-07 -1.42E-08 -1.09E-08
NHWD kg 1.23E-01 8.64E-05 9.13E-01 2.37E-05 0 0 2.25E-01 4.47E+01 -1.96E-02 -1.83E-02
RWD kg 2.93E-03 9.94E-07 8.09E-05 2.76E-07 0 0 1.98E-04 7.93E-04 -3.85E-03 -3.88E-03
CRU kg 0 0 0 0 0 0 0 0 0 0
MFR kg 0 0 1.37E-02 0 0 0 0 0 0 0
MER kg 0 0 1.56E-02 0 0 0 2.35E+00 0 0 0
EEE MJ 0 0 3.39E-01 0 0 0 1.25E+01 1.26E+01 0 0
EET MJ 0 0 1.56E-01 0 0 0 7.85E+00 0 0 0
HWD = Hazardous waste disposed; NHWD = Non-hazardous waste disposed; RWD = Radioactive waste disposed; CRU = Components for re-use;
MFR = Materials for recycling; MER = Materials for energy recovery; EEE = Exported electrical energy; EET = Exported thermal energy
Disclaimer 1 – for the indicator 'Potential Human exposure efficiency relative to U235'. This impact category deals mainly with the
eventual impact of low-dose ionizing radiation on human health of the nuclear fuel cycle. It does not consider effects due to possible
4 Environmental Product Declaration - Stiferite - Stiferite BB average thick panel
nuclear accidents, occupational exposure or radioactive waste disposal in underground facilities. Potential ionizing radiation from the
soil, radon and from some construction materials is also not measured by this indicator.
Disclaimer 2 – for the indicators 'abiotic depletion potential for non-fossil resources', 'abiotic depletion potential for fossil resources',
'water (user) deprivation potential, deprivation-weighted water consumption', 'potential comparative toxic unit for ecosystems', 'potential
comparative toxic unit for humans – cancerogenic', 'Potential comparative toxic unit for humans - not cancerogenic', 'potential soil
quality index'. The results of this environmental impact indicator shall be used with care as the uncertainties on these results are high
as there is limited experience with the indicator.
References
Standards
ISO 14001
EN 15804 ISO 14001: 2015 Environmental management systems
EN 15804:2012-04+A1 2013, Sustainability of construction
works — Environmental Product Declarations — Core rules for ISO 45001
the product category of construction products. ISO 45001: 2018 Occupational health and safety management
systems
ISO 14025
EN ISO 14025:2011-10, Environmental labels and declarations
— Type III environmental declarations — Principles and Further References
procedures.
BNB
IBU 2016 Bewertungssystem Nachhaltiges Bauen (en: assessment
Institut Bauen und Umwelt e.V.: General Programme system sustainable building)
Instructions for the Preparation of EPDs at the Institut Bauen https://www.bbsr.bund.de/BBSR/EN/RP/FutureBuilding/2SustainableBuildingQuality/2009/ServiceLife/01_Start_dossier.html?
und Umwelt e.V. Version 1., Berlin: Institut Bauen und Umwelt n=391866&notFirst=true&docId=390900
e.V., 2016.
www.ibu-epd.com Candidate List
https://echa.europa.eu/it/candidate-list-table (date 17.11.2020)
EN 13165
EN 13165:2012+A2:2016 Thermal insulation products for CLIMA 2019
buildings - Factory made rigid polyurethane foam (PU) CLIMA 2019 PaperPolyurethane 'Environmental Impacts for a
products - Specification Polyurethane Panel' E. Guolo, F. Cappelletti, P. Romagnoni, F.
Raggiotto
EN 826
EN 826:2013 Determination of Compression Behavior of GaBi 9 2020
Thermal Insulation Products GaBi 9: Documentation of GaBi 9: Software-System and
Database for Life Cycle Engineering. Copyright, TM. Stuttgart,
EN 1607 Leinfelden-Echterdingen, 1992-2020
EN 1607: 2013 Thermal insulating products for building http://www.gabi-software.com
applications. Determination of tensile strength perpendicular to
faces PANGPP 2017
Piano d' Azione Nazionale sul Green Public Procurement
EN 12087 (PANGPP) – Gazzetta Ufficiale della Repubblica Italiana, Serie
EN 12087:2013 Thermal insulating products for building Generale n.17, 11-10-2017,
applications. Determination of long term water absorption by http://www.minambiente.it/sites/default/files/archivio/allegati/GPP/GPP_CAM_Edilizia.pdf
immersion.
PCR Part A
EN 1609 les for Building-Related Products and Services. Part A:
EN 1609: Thermal insulating products for building applications. Calculation Rules for the Life Cycle Assessment and
Determination of short term water absorption by partial Requirements on the Background Report. Version 06.2017
immersion.
PCR Part B
EN 12086 PCR Guidance-Texts for Building-Related Products and
EN 12086: 2013 Thermal insulating products for building Services; Part B: Requirements on the EPD for Insulating
applications. Determination of water vapour transmission materials made of foam plastics; Institute Construction and
properties. Environment e.V. (IBU). Version 06.2017
https://epd-online.com
EN 11925
EN 11925:2010 Reaction to fire tests. Ignitability of products REACH
subjected to direct impingement of flame. Single-flame source REACH Registration, Evaluation, Authorization and Restriction
test. of Chemical, 2007
ISO 9001 CLIMA 2019_PaperPolyurethane
ISO 9001:2015 Quality management
5 Environmental Product Declaration - Stiferite - Stiferite BB average thick panel
Publisher
Institut Bauen und Umwelt e.V. +49 (0)30 3087748- 0
Hegelplatz 1 info@ibu-epd.com
10117 Berlin www.ibu-epd.com
Germany
Programme holder
Institut Bauen und Umwelt e.V. +49 (0)30 3087748- 0
Hegelplatz 1 info@ibu-epd.com
10117 Berlin www.ibu-epd.com
Germany
Author of the Life Cycle Assessment
thinkstep Italy +39 0544 467132
Via Bovini 43 info@thinkstep.com
48123 Ravenna www.thinkstep.com
Italy
Owner of the Declaration
Stiferite +39 049 8997911
Viale Navigazione Interna 54 info@stiferite.com
35129 Padova www.stiferite.com
Italy
6 Environmental Product Declaration - Stiferite - Stiferite BB average thick panel
