ENVIRONMENTAL PRODUCT DECLARATION
as per ISO 14025 and EN 15804+A2
Owner of the Declaration Vebe Floorcoverings B.V.
Programme holder Institut Bauen und Umwelt e.V. (IBU)
Publisher Institut Bauen und Umwelt e.V. (IBU)
Declaration number EPD-VEB-20220242-CBB1-EN
Issue date 30.11.2022
Valid to 29.11.2027
Needled carpet tiles
with a maximum pile weight of 1790 g/m2, and a pile
composition of 80% polypropylene and 20% polyester,
NSF foam backing
Vebe Floorcoverings B. V.
www.ibu-epd.com | https://epd-online.com
Umwelt Produktdeklaration Name des Herstellers – Name des Produkts
General Information
Vebe Floorcoverings B.V. Needled carpet tiles
with a maximum pile weight of 1790
g/m2 and a pile composition of 80%
polypropylene and 20% polyester,
NSF foam backing
Programme holder Owner of the declaration
IBU – Institut Bauen und Umwelt e.V. Vebe Floorcoverings B.V.
Hegelplatz 1 Inslag 12
10117 Berlin 8281 JV, Genemuiden
Germany Netherlands
www.vebe.eu
Declaration number Declared product / declared unit
EPD-VEB-20220242-CBB1-EN 1 m² needled tiles, PP and PET pile material with a
NSF foam backing
This declaration is based on the product Scope:
category rules: The manufacturer declaration applies to a group of
Floor coverings, 02/2018 needled carpet tiles with a foam backing. The pile
(PCR checked and approved by the SVR) material consists of minimum 80% polypropylene and
maximum 20% of polyester. The maximum total pile
weight is 1790 g/m2. The products are produced in
Issue date
Genemuiden, Netherlands.
30.11.2022
LCA results for products with a maximum total pile
weight of 1150 g/m2 can be taken from the
Valid to
corresponding tables of the annexe. Specific data for
29.11.2027 every product within the declared group of products in
relation to its total pile weight can be calculated by
using equation 1 given in the annexe (see annexe
chapter: 'General Information on the annexe'). The
declaration is only valid in conjunction with a valid
GUT-PRODIS license of the product.
The owner of the declaration shall be liable for the
underlying information and evidence; the IBU shall not
be liable with respect to manufacturer information, life
cycle assessment data and evidences.
The EPD was created according to the specifications
of EN 15804+A2. In the following, the standard will be
simplified as EN 15804.
Verification
The standard EN 15804 serves as the core PCR
Independent verification of the declaration and data
according to ISO 14025:2011
Dipl. Ing. Hans Peters internally x externally
(chairman of Institut Bauen und Umwelt e.V.)
Dr. Alexander Röder Angela Schindler
(Managing Director Institut Bauen und Umwelt e.V.)) (Independent verifier)
Product
Product description/Product definition
The declaration applies to needled carpet tiles with a For the placing on the market of the specific product in
foam backing. The pile material consists of at least the European Union/European Free Trade Association
80% Polypropylene and max. 20% of polyester which (EU/EFTA) (with the exception of Switzerland)
is 100% recycled. Maximum total pile weight is 1790 Regulation (EU) No. 305/2011 Construction Product
g/m2. The maximum recycled content of the carpet is Regulation (CPR) applies. The product needs a
12% having 20% polyester in the pile material and a Declaration of Performance (DoP) taking into
maximum total pile weight of 1790 g/m2.
2 Environmental Product Declaration Vebe Floorcoverings B. V. – Needled carpet tiles, yarn mixture of 80% polypropylene,
20% polyester and an NSF foam backing
consideration EN 14041:2018-05, Resilient, textile and Name Value Unit
laminate floor coverings - Essential characteristics, and Polypropylene 48.5 %
the CE-marking. The DoP of the product can be found Polyester 12.1 %
on the manufacturer's technical information section. SBR Latex 38.2 %
For the application and use of the product the Additives 1.2 %
respective national provisions apply.
The specific product coverd by the EPD contains
Application substances listed in the ECHA candidate list
The use class of the specific product as defined in (08.07.2021) or other carcinogenic, mutagenic or
EN 1307 can be found in the Product Information reprotoxic (CMR) substances in categories 1A or 1B
System (PRODIS) using the PRODIS registration which are not on the candidate list exceeding 0.1
number of the product. percentage by mass: no
The products are registered in the GUT-PRODIS
Technical Data Information System. The PRODIS system ensures the
The technical data describes a fictitious worst-case compliance with limitations of various chemicals and
product representing all products with the described Volatile Organic Compound (VOC)-emissions and a
characteristics. ban on the use of all substances that are listed as
'Substances of Very High Concern' (SVHC) under
Constructional data according to EN 1307 REACH.
Name Value Unit
Product Form Tiles - Reference service life
Type of manufacture Needled carpet - The service life of textile floor coverings strongly
Yarn type 80% PP / 20% PET - depends on the correct installation taking into account
Total carpet weight 2952 g/m2 the declared use classification and the adherence to
Secondary backing foam backing - cleaning and maintenance instructions.
A calculation of the reference service life according to
ISO 15686 is not possible.
Performance data of the product in accordance with Alternatively, a reference service life of 10 years can
the declaration of performance with respect to its be assumed, during which the functional and visual
essential characteristics according to EN 14041: 2018- quality is guaranteed (BNB, Nutzungsdauer von
05, Resilient, textile and laminate floor coverings - Bauteilen). The technical service life can be
Essential characteristics. significantly longer.
Additional product properties in accordance with EN
1307 can be found on the Product Information System
PRODIS using the PRODIS registration number of the
product (www.pro-dis.info) or on the manufacturer's
technical information section.
Base materials/Ancillary materials
LCA: Calculation rules
Declared Unit 1 - landfill disposal
2 - municipal waste incineration
3 - recovery in a cement plant
Name Value Unit
Declared unit 1 m2 A1-A3 Production:
Grammage 2952 kg/m2 Energy supply and production of the basic material,
The declared unit refers to 1 m2 produced textile floor processing of secondary material, auxiliary material,
covering. The Output of module A5 'Assembly' is 1 m2 transport of the material to the manufacturing site,
installed textile floor covering. emissions, waste water treatment, packaging material
The layer thickness of the specific product covered by and waste processing up to the landfill disposal of
the EPD can be found on the Product Information residual waste (except radioactive waste). Benefits for
System PRODIS using the PRODIS registration generated electricity and steam due to the incineration
number of the product (www.pro-dis.info) or on the of production waste are aggregated.
manufacturer's technical information section. Biogenic carbon that is stored in renewable material
(packaging paper) is taken into account as well as the
associated carbon dioxide uptake from the air from
which this biogenic carbon comes.
System boundary
A4 Transport:
Type of EPD: Cradle-to-grave Transport of the packed textile floor covering
System boundaries of modules A, B, C, D: from factory gate to the place of installation.
Modules C3, C4 and D are indicated separately for
three end-of-life scenarios: A5 Installation:
Installation of the textile floor covering, processing of
installation waste and packaging waste up to the
3 Environmental Product Declaration Vebe Floorcoverings B. V. – Needled carpet tiles, yarn mixture of 80% polypropylene,
20% polyester and an NSF foam backing
landfill disposal of residual waste (except radioactive Transport of the carpet waste to a landfill, to the
waste), the production of the amount of carpet that municipal waste incineration plant (MWI) or to the
occurs as installation waste including its transport to waste collection facility for recycling.
the place of installation.
Generated electricity and steam due to the incineration C3 Waste processing:
of waste are listed in the result table as exported C3-1: Landfill disposal needs no waste processing.
energy. C3-2: Impact from waste incineration (plant with
Biogenic carbon that is stored in renewable materials R1>0.6), generated electricity and steam are listed in
in packaging paper is released as carbon dioxide the result table as exported energy.
emissions into the air at the end of life in module A5. C3-3: Collection of the carpet waste for recovery in the
Preparation of the floor and auxiliary materials cement industry, waste processing (granulating),
(adhesives, fixing agents, PET connectors) are beyond transport to the cement plant, emissions from the
the system boundaries and not taken into account. incineration.
B1 Use: C4 Disposal
Indoor emissions during the use stage. After the first C4-1: Impact from landfill disposal,
year, no product-related Volatile Organic Compound C4-2: The carpet waste leaves the system in
(VOC) emissions are relevant due to the known VOC module C3-2,
decay curves of the product. C4-3: The pre-processed carpet waste leaves the
system in module C3-3.
B2 Maintenance:
Cleaning of the textile floor covering for a period of 1 D Recycling potential:
year: Calculated benefits result from materials exclusive
Vacuum cleaning – electricity supply secondary materials (net materials).
Wet cleaning – electricity, water consumption, D-A5: Benefits for generated energy due
production of the cleaning agent, waste water to incineration of packaging and installation waste
treatment. (incineration plant with R1 > 0.6),
The declared values in this module have to be D-1: Benefits for generated energy due to landfill
multiplied by the assumed service life of the floor disposal of carpet waste at the end-of-life,
covering in the building in question. D-2: Benefits for generated energy due to incineration
of carpet waste at the end-of-life (incineration plant
B3 - B5: with R1 > 0.6),
The modules are not relevant within the assumed D-3: Benefits for saved fossil energy and saved
reference service life of 10 years. inorganic material due to recovery of the carpet in a
cement plant.
B6 - B7:
No energy and water input are required for the Comparability
operation of the carpet in the use stage. The modules Basically, a comparison or an evaluation of EPD data
do not cause any environmental impact. is only possible if all the data sets to be compared
were created according to EN 15804 and the building
C1 De-construction: context, respectively the product-specific
The floor covering is de-constructed manually and no characteristics of performance, are taken into account.
additional environmental impact is caused.
Background data are taken from the GaBi database,
C2 Transport: 2021-2. Remaining data gaps are covered by the
ecoinvent 3.7 database, 2020.
LCA: Scenarios and additional technical information
Characteristic product properties
Information on biogenic Carbon
Installation in the building (A5)
Name Value Unit Name Value Unit
Biogenic Carbon Content in Material loss 0.089 kg
accompanying packaging at factory 0.001 kg C Polyethylene packaging waste and installation waste
gate are considered to be incinerated in a municipal waste
1 kg biogenic Carbon is equivalent to 44/12 kg of CO incineration plant. Cardboard packaging waste is going
2
to be recycled.
Preparation of the floor and auxiliaries (adhesives,
fixing agents, PET connectors etc.) are not taken into
Transport to the construction site (A4) account.
Name Value Unit
Litres of fuel (truck, EURO 0-6 Maintenance (B2)
0.0069 l/100km
mix) The values for cleaning refer to 1 m2 floor covering per
Transport distance 700 km year.
Capacity utilisation (including Depending on the application based on ISO 10874, the
55 %
empty runs) technical service life recommended by the
manufacturer and the anticipated strain on the floor by
customers, the case-specific useful life can be
4 Environmental Product Declaration Vebe Floorcoverings B. V. – Needled carpet tiles, yarn mixture of 80% polypropylene,
20% polyester and an NSF foam backing
established. Based on this useful life the effects of for lignite (68.8 %), hard coal (23.6 %) and petrol coke
module B2 need to be calculated in order to obtain the (7.6 %). The inorganic material is substantially
overall environmental impacts. integrated into the cement clinker and substitutes for
the original material input. VDZ e.V.
Name Value Unit
Number
Maintenance cycle (vacuum cleaning) 208
/year
Number
Maintenance cycle (wet cleaning) 1,5
/year
Water consumption (wet cleaning) 0.004 m3
Cleaning agent (wet cleaning) 0.09 kg
Electricity consumption 0.314 kWh
For further information on cleaning and maintenance
see www.vebe.eu
Service life
Name Value Unit
Life Span (according to BBSR) 10 a
Corresponds to
Declared product properties (at the
-
the gate) and finishes specifications of
EN 1307
An assumed quality of work, when Conforms to the
installed in accordance with the manufacturer's -
manufacturer’s instructions instructions
Use in areas
defined by the
Usage conditions, e.g. frequency
use class -
of use, mechanical exposure
according to EN
1307
Maintenance e.g. required According to the
frequency, type and quality and manufacturers -
replacement of components instructions
End of Life (C1-C4)
Three different end-of-life scenarios are declared and
the results are indicated separately in module C.
Each scenario is calculated as a 100% scenario.
Scenario 1: 100 % landfill disposal
Scenario 2: 100 % municipal waste incineration (MWI)
with R1>0.6
Scenario 3: 100 % recovery in the cement industry
If combinations of these scenarios have to be
calculated this should be done according to the
following scheme:
EOL-impact = x % impact (Scenario 1)
+ y % impact (Scenario 2)
+ z % impact (Scenario 3)
with x % + y % + z % = 100 %
Name Value Unit
Collected as mixed construction
2.952 kg
waste (scenario's 1 and 2)
Collected separately (scenario 3) 2.952 kg
Landfilling (scenario 1) 2.952 kg
Energy recovery (scenario 2) 2.952 kg
Energy recovery (scenario 3) 2.952 kg
Recycling (scenario 3) 0 kg
Reuse, recovery and/or recycling potentials (D),
relevant scenario information
Recovery or recycling potentials due to the three end-
of-life scenarios (module C) are indicated separately.
Recycling in the cement industry (scenario 3)
The organic material of the carpet is used as an
alternative fuel in a cement kiln. It mainly substitutes
5 Environmental Product Declaration Vebe Floorcoverings B. V. – Needled carpet tiles, yarn mixture of 80% polypropylene,
20% polyester and an NSF foam backing
LCA: Results
The LCA results refer to all declared products with a maximum total pile weight of 1790 g/m2. LCA results for
products with a maximum total pile weight of 1150 g/m2 can be taken from the corresponding tables of the
annexe. Results for specific products with any other total pile weight can be calculated by using equation 1 given
in the annexe (see annexe chapter: 'General Information on the annexe'). The declared result figures in module
B2 have to be multiplied by the assumed service life (in years) of the floor covering in the building under
consideration. Information on non-relevant modules: Modules B3 - B7 are not relevant during the service life of
the carpet. Modules C1, C3/1, C4/2 and C4/3 cause no additional impact (see chapter "LCA: Calculation rules" in
this document). All these modules are declared and marked as 'modules not relevant/declared'. Module C2
represents the transport for scenarios 1, 2 and 3. Column D represents module D/A5.
DESCRIPTION OF THE SYSTEM BOUNDARY (X = INCLUDED IN LCA; ND = MODULE OR INDICATOR NOT
DECLARED; MNR = MODULE NOT RELEVANT)
BENEFITS AND
CONSTRUCTI LOADS
PRODUCT STAGE ON PROCESS USE STAGE END OF LIFE STAGE BEYOND THE
STAGE SYSTEM
BOUNDARIES
6 Environmental Product Declaration Vebe Floorcoverings B. V. – Needled carpet tiles, yarn mixture of 80% polypropylene,
20% polyester and an NSF foam backing
lairetam
waR
ylppus tropsnarT
gnirutcafunaM
eht
morf
tropsnarT
etis
eht
ot
etag
ylbmessA esU
ecnanetniaM
riapeR
tnemecalpeR tnemhsibrufeR
ygrene
lanoitarepO esu
retaw
lanoitarepO esu
noitcurtsnoc-eD
noitilomed tropsnarT
gnissecorp
etsaW
lasopsiD -esueR -yrevoceR -gnilcyceR laitnetop
A1 A2 A3 A4 A5 B1 B2 B3 B4 B5 B6 B7 C1 C2 C3 C4 D
X X X X X X X MNR MNR MNR ND ND X X X X X
RESULTS OF THE LCA - ENVIRONMENTAL IMPACT according to EN 15804+A2: 1 m² floor covering
Core Indicator Unit A1-A3 A4 A5 B1 B2 C1 C2 C3/2 C3/3 C4/1 D D/1 D/2 D/3
-
GWP-total [kg CO2-Eq.] 8.04E+01.76E-1 4.58E-10.00E+04.16E-10.00E+01.00E-26.78E+06.82E+02.07E-1-7.62E-20.00E+0 2.50E+0-4.72E-1
-
GWP-fossil [kg CO2-Eq.] 8.01E+01.72E-1 4.52E-10.00E+02.15E-10.00E+09.84E-36.77E+06.81E+02.07E-1-7.58E-20.00E+0 2.49E+0-4.71E-1
GWP-biogenic [kg CO2-Eq.] 2.12E-2 2.23E-3 5.72E-30.00E+04.16E-30.00E+01.27E-4 3.13E-4 7.68E-40.00E+0-3.88E-40.00E+0-1.27E-2-5.34E-4
GWP-luluc [kg CO2-Eq.] 5.50E-3 9.76E-4 1.97E-40.00E+01.96E-10.00E+05.57E-5 2.59E-5 1.68E-4 1.02E-4-8.35E-60.00E+0-2.74E-4-1.97E-4
1.05E- 1.48E- 5.99E- 4.82E- 7.05E- 2.81E- -5.14E- -1.68E- -8.72E-
ODP [kg CFC11-Eq.] 4.93E-9 0.00E+03.42E-80.00E+0 0.00E+0
14 10 16 13 13 13 13 11 13
AP [mol H+-Eq.] 1.70E-2 1.04E-3 5.81E-40.00E+08.32E-40.00E+05.95E-5 1.29E-3 1.47E-3 6.20E-4-9.99E-50.00E+0-3.27E-3-1.37E-3
EP-freshwater [kg P-Eq.] 2.56E-5 5.23E-7 7.89E-70.00E+05.19E-60.00E+02.98E-8 1.94E-7 3.13E-7 3.91E-5-1.05E-70.00E+0-3.43E-6-4.66E-7
EP-marine [kg N-Eq.] 4.68E-3 5.12E-4 1.69E-40.00E+01.97E-40.00E+02.92E-5 4.12E-4 4.93E-4 1.37E-4-2.71E-50.00E+0-8.88E-4-4.64E-4
EP-terrestrial [mol N-Eq.] 5.00E-2 5.67E-3 1.86E-30.00E+02.83E-30.00E+03.23E-4 5.85E-3 6.74E-3 1.51E-3-2.90E-40.00E+0-9.51E-3-5.08E-3
POCP [kg NMVOC-Eq.]1.58E-2 9.68E-4 5.38E-4 4.18E-4 9.83E-40.00E+05.52E-5 1.12E-3 1.27E-3 4.41E-4-7.58E-50.00E+0-2.48E-3-1.44E-3
8.35E-
ADPE [kg Sb-Eq.] 1.27E-6 1.46E-8 3.90E-80.00E+02.30E-70.00E+0 1.18E-8 1.80E-8 1.45E-8-1.15E-80.00E+0-3.76E-7-4.20E-8
10
- - -
ADPF [MJ] 2.41E+22.34E+07.35E+00.00E+05.90E+00.00E+01.34E-11.33E+01.94E+02.97E+0 0.00E+0
1.29E+0 4.23E+17.67E+1
[m³ world-Eq
WDP 9.89E+01.57E-3 3.17E-10.00E+09.99E-20.00E+08.94E-5 6.70E-1 6.74E-1-2.22E-3-8.01E-30.00E+0-2.62E-1-7.67E-2
deprived]
GWP = Global warming potential; ODP = Depletion potential of the stratospheric ozone layer; AP = Acidification potential of land and water; EP =
Caption Eutrophication potential; POCP = Formation potential of tropospheric ozone photochemical oxidants; ADPE = Abiotic depletion potential for non-
fossil resources; ADPF = Abiotic depletion potential for fossil resources; WDP = Water (user) deprivation potential
RESULTS OF THE LCA - INDICATORS TO DESCRIBE RESOURCE USE according to EN 15804+A2: 1 m²
floor covering
Indicator Unit A1-A3 A4 A5 B1 B2 C1 C2 C3/2 C3/3 C4/1 D D/1 D/2 D/3
PERE [MJ] 1.90E+1 1.33E-1 5.84E-1 0.00E+0 3.69E+0 0.00E+0 7.59E-3 3.05E-1 4.76E-1 2.44E-1 -3.55E-1 0.00E+0 -1.16E+1-5.23E-1
PERM [MJ] 7.00E-3 0.00E+0 0.00E+0 0.00E+0 0.00E+0 0.00E+0 0.00E+0 -7.00E-3 -7.00E-3 0.00E+0 0.00E+0 0.00E+0 0.00E+0 0.00E+0
PERT [MJ] 1.90E+1 1.33E-1 5.84E-1 0.00E+0 3.69E+0 0.00E+0 7.59E-3 2.98E-1 4.69E-1 2.44E-1 -3.55E-1 0.00E+0 -1.16E+1-5.23E-1
PENRE [MJ] 1.55E+2 2.35E+0 7.39E+0 0.00E+0 5.90E+0 0.00E+0 1.34E-1 8.82E+1 8.88E+1 2.97E+0 -1.29E+0 0.00E+0 -4.23E+1-7.67E+1
PENRM [MJ] 8.69E+1 0.00E+0 -3.70E-2 0.00E+0 0.00E+0 0.00E+0 0.00E+0 -8.68E+1-8.68E+1 0.00E+0 0.00E+0 0.00E+0 0.00E+0 0.00E+0
PENRT [MJ] 2.41E+2 2.35E+0 7.36E+0 0.00E+0 5.90E+0 0.00E+0 1.34E-1 1.33E+0 1.94E+0 2.97E+0 -1.29E+0 0.00E+0 -4.23E+1-7.67E+1
SM [kg] 3.63E-1 0.00E+0 1.09E-2 0.00E+0 0.00E+0 0.00E+0 0.00E+0 0.00E+0 0.00E+0 0.00E+0 0.00E+0 0.00E+0 0.00E+0 0.00E+0
RSF [MJ] 0.00E+0 0.00E+0 0.00E+0 0.00E+0 0.00E+0 0.00E+0 0.00E+0 0.00E+0 0.00E+0 0.00E+0 0.00E+0 0.00E+0 0.00E+0 0.00E+0
NRSF [MJ] 0.00E+0 0.00E+0 0.00E+0 0.00E+0 0.00E+0 0.00E+0 0.00E+0 0.00E+0 0.00E+0 0.00E+0 0.00E+0 0.00E+0 0.00E+0 0.00E+0
FW [m³] 2.44E-1 1.50E-4 7.79E-3 0.00E+0 3.34E-3 0.00E+0 8.58E-6 1.57E-2 1.59E-2 3.48E-5 -3.39E-4 0.00E+0 -1.11E-2 -6.66E-3
PERE = Use of renewable primary energy excluding renewable primary energy resources used as raw materials; PERM = Use of
renewable primary energy resources used as raw materials; PERT = Total use of renewable primary energy resources; PENRE = Use of
non-renewable primary energy excluding non-renewable primary energy resources used as raw materials; PENRM = Use of non-
Caption
renewable primary energy resources used as raw materials; PENRT = Total use of non-renewable primary energy resources; SM = Use
of secondary material; RSF = Use of renewable secondary fuels; NRSF = Use of non-renewable secondary fuels; FW = Use of net fresh
water
RESULTS OF THE LCA – WASTE CATEGORIES AND OUTPUT FLOWS according to EN 15804+A2:
1 m² floor covering
Indicator Unit A1-A3 A4 A5 B1 B2 C1 C2 C3/2 C3/3 C4/1 D D/1 D/2 D/3
HWD [kg] 8.66E-6 1.12E-11 2.60E-7 0.00E+0 4.19E-5 0.00E+0 6.41E-131.28E-101.53E-104.58E-10-1.75E-100.00E+0 -5.72E-9-1.28E-10
NHWD [kg] 8.81E-2 3.36E-4 9.32E-3 0.00E+0 7.30E-3 0.00E+0 1.92E-5 2.22E-1 2.22E-1 2.94E+0 -6.52E-4 0.00E+0 -2.14E-2 -1.47E-3
RWD [kg] 7.54E-3 2.89E-6 2.28E-4 0.00E+0 3.76E-4 0.00E+0 1.65E-7 6.97E-5 1.14E-4 3.65E-5 -1.02E-4 0.00E+0 -3.34E-3 -1.05E-4
CRU [kg] 0.00E+0 0.00E+0 0.00E+0 0.00E+0 0.00E+0 0.00E+0 0.00E+0 0.00E+0 0.00E+0 0.00E+0 0.00E+0 0.00E+0 0.00E+0 0.00E+0
MFR [kg] 0.00E+0 0.00E+0 3.40E-3 0.00E+0 0.00E+0 0.00E+0 0.00E+0 0.00E+0 0.00E+0 0.00E+0 0.00E+0 0.00E+0 0.00E+0 0.00E+0
MER [kg] 0.00E+0 0.00E+0 0.00E+0 0.00E+0 0.00E+0 0.00E+0 0.00E+0 0.00E+0 0.00E+0 0.00E+0 0.00E+0 0.00E+0 0.00E+0 0.00E+0
EEE [MJ] 0.00E+0 0.00E+0 3.77E-1 0.00E+0 0.00E+0 0.00E+0 0.00E+0 1.24E+1 0.00E+0 0.00E+0 0.00E+0 0.00E+0 0.00E+0 0.00E+0
EET [MJ] 0.00E+0 0.00E+0 6.76E-1 0.00E+0 0.00E+0 0.00E+0 0.00E+0 2.22E+1 9.50E+1 0.00E+0 0.00E+0 0.00E+0 0.00E+0 0.00E+0
HWD = Hazardous waste disposed; NHWD = Non-hazardous waste disposed; RWD = Radioactive waste disposed; CRU = Components
Caption for re-use; MFR = Materials for recycling; MER = Materials for energy recovery; EEE = Exported electrical energy; EET = Exported
thermal energy
RESULTS OF THE LCA – additional impact categories according to EN 15804+A2-optional:
1 m² floor covering
Indicator Unit A1-A3 A4 A5 B1 B2 C1 C2 C3/2 C3/3 C4/1 D D/1 D/2 D/3
[Disease -8.27E-
PM 1.59E-7 6.02E-9 5.21E-9 0.00E+0 6.84E-8 0.00E+03.44E-10 8.23E-9 9.36E-9 5.96E-9 0.00E+0 0.00E+0 -1.78E-8
Incidence] 10
[kBq U235-
IRP 8.32E-1 4.23E-4 2.53E-2 0.00E+0 6.78E-2 0.00E+0 2.42E-5 1.12E-2 1.87E-2 5.38E-3 -1.72E-2 0.00E+0 0.00E+0 -9.01E-3
Eq.]
ETP-fw [CTUe] 1.23E+2 1.62E+0 3.76E+0 3.60E-3 2.69E+0 0.00E+0 9.27E-2 6.80E-1 1.03E+0 2.91E+0 -2.84E-1 0.00E+0 0.00E+0-1.29E+1
-1.30E- -1.14E-
HTP-c [CTUh] 3.80E-9 3.28E-111.17E-100.00E+06.21E-100.00E+01.87E-126.00E-116.82E-111.30E-10 0.00E+0 0.00E+0
11 10
-5.00E-
HTP-nc [CTUh] 2.56E-7 1.95E-9 7.85E-9 2.60E-11 9.46E-9 0.00E+01.11E-10 3.53E-9 3.93E-9 1.09E-8 0.00E+0 0.00E+0 -5.74E-9
10
SQP [-] ND ND ND ND ND ND ND ND ND ND ND ND ND ND
PM = Potential incidence of disease due to PM emissions; IR = Potential Human exposure efficiency relative to U235; ETP-fw = Potential
Caption comparative Toxic Unit for ecosystems; HTP-c = Potential comparative Toxic Unit for humans (cancerogenic); HTP-nc = Potential
comparative Toxic Unit for humans (not cancerogenic); SQP = Potential soil quality index
No substantiated values can be given for the SQP indicator with the existing database.
The result figures given in module B2 refer to a period of 1 year because a reference service life is not declared.
They have to be multiplied by the assumed service life (in years) of the floor covering in the building under
consideration.
Disclaimer 1 – for the indicator “Potential Human exposure efficiency relative to U235”.
This impact category deals mainly with the eventual impact of low dose ionizingradiation on human health of the
nuclear fuel cycle. It does not consider effects due to possible nuclear accidents, occupational exposure or to
radioactive waste disposal in undergroundfacilities. Potential ionizing radiation from the soil, radon and from some
construction materials is also not measured by this indicator.
Disclaimer 2 – for the indicators “abiotic depletion potential for non-fossil resources”, “abiotic depletion potential
for fossil resources”, “water (user) deprivation potential, deprivation-weighted water consumption”, “potential
comparative toxic unit for ecosystems”, “potential comparative toxic unit for humans – cancerogenic”, “Potential
comparative toxic unit for humans - not cancerogenic”, “potential soil quality index”.
The results of this environmental impact indicator shall be used with care as the uncertainties on these results are
high as there is limited experience with the indicator.
References
EN 1307 floor coverings – Environmental product declarations –
DIN EN 1307: 2014+A1:2016+A2:2018-05: Textile Product category rules
floor coverings - Classification
ISO 10874
EN 13501-1 DIN EN ISO 10874: 2012+A1:2021-04: Resilient,
DIN EN 13501-1:2019-05: Fire classification of textile and laminate floor coverings - Classification
construction products and building elements - Part 1:
Classification using data from reaction to fire tests ISO 14025
DIN EN /ISO 14025:2011-10/, Environmental labels
EN 14041 and declarations — Type III environmental
DIN EN 14041: 2018-05 and DIN EN 14041: 2008-05: declarations — Principles and procedures
Resilient, textile and laminate floor coverings -
Essential characteristics
ISO 14040
EN 15804 DIN EN ISO 14040:2006+A1:2020 Environmental
DIN EN 15804:2012+A2:2019 + AC:2021, management - Life cycle assessment - Principles and
Sustainability of construction works — Environmental framework
Product Declarations — Core rules for the product
category of construction products ISO 14044
DIN EN ISO 14044:2006+A1:2018+A2:2020
EN 16810 Environmental management - Life cycle assessment -
DIN EN 16810: 2017-08: Resilient, textile and laminate Requirements and guidelines
7 Environmental Product Declaration Vebe Floorcoverings B. V. – Needled carpet tiles, yarn mixture of 80% polypropylene,
20% polyester and an NSF foam backing
ISO 15686 GaBi database
ISO 15686: Buildings and constructed assets - GaBi Software-System and Database for Life Cycle
Service life planning Engineering, thinkstep AG, Leinfelden-Echterdingen,
ISO 15686-1: 2011-05: Part 1: General principles and 2022-1
framework
ISO 15686-2: 2012-05: Part 2: Service life prediction PCR Part A
procedures Product Category Rules for Building-Related Products
ISO 15686-7: 2017-04: Part 7: Performance and Services Part A: Calculation Rules for the Life
evaluation for feedback of service life data Cycle Assessment and Requirements on the Project
from practice Report according to EN 15804+A2:2019, V1.1, Berlin:
ISO 15686-8: 2008-06: Part 8: Reference service life Institut Bauen und Umwelt e.V. (IBU), January 2021
and service-life estimation
PCR Part B
Regulation (EU) No. 305/2011 Product Category Rules for Building-Related Products
Regulation No. 305/2011 Construction Products and Services
Regulation (CPR) of the European Council and of the Part B: Requirements on the EPD for floor coverings,
European Parliament, April 2011 V1.2, Berlin: Institut Bauen und Umwelt e.V. (IBU),
February 2018
General Instructions for the IBU-EPD Program
General Instructions for the EPD-Program of the PRODIS
Institut Bauen und Umwelt e.V., The Preparation of Product Information System (PRODIS) of the
Environmental Product Declarations - EPDs, version European Carpet Industry, Gemeinschaft
2.0, Institut Bauen und Umwelt e.V., Berlin, January umweltfreundlicher Teppichboden e.V (GUT) and
2021, www.ibu-epd.de European Carpet and Rug Association
(ECRA), http://www.pro-dis.info
BNB, Nutzungsdauer von Bauteilen
Bewertungssystem Nachhaltiges Bauen (BNB), REACH
Nutzungsdauer von Bauteilen, Bundesministerium des Regulation (EC) No 1907/2006 of the European
Inneren, für Bau und Heimat, 24.02.2017 Parliament and of the Council of 18 December 2006
concerning the Registration, Evaluation, Authorisation
ECHA candidate list and Restriction of Chemicals (REACH), June 2017,
Candidate List of substances of very high concern last update: 08.07.2021
(SVHCs) for authorisation, 08.07.2021, European
Chemicals Agency (ECHA), Helsinki, Finland VDZ e.V.
Association of German Cement Works, Ed. Environ-
mental Data of the German Cement Industry 2020
ecoinvent
ecoinvent, Zurich, Switzerland, database version 3.7,
published September 2020
8 Environmental Product Declaration Vebe Floorcoverings B. V. – Needled carpet tiles, yarn mixture of 80% polypropylene,
20% polyester and an NSF foam backing
Publisher
Institut Bauen und Umwelt e.V. Tel +49 (0)30 3087748- 0
Hegelplatz 1 Fax +49 (0)30 3087748- 29
10117 Berlin Mail info@ibu-epd.com
Germany Web www.ibu-epd.com
Programme holder
Institut Bauen und Umwelt e.V. Tel +49 (0)30 - 3087748- 0
Hegelplatz 1 Fax +49 (0)30 – 3087748 - 29
10117 Berlin Mail info@ibu-epd.com
Germany Web www.ibu-epd.com
Author of the Life Cycle
Assessment Tel +49 (0)241 96843 410
Gemeinschaft umweltfreundlicher Fax +49 (0)241 96843 400
Teppichboden (GUT) e.V. Mail mail@gut-ev.de
Schönebergstraße 2 Web www.gut-ev.org
52068 Aachen
Germany
Owner of the Declaration
Vebe Floorcoverings B.V. Tel +31 (0)38 3853200
Inslag 12 Fax +31 (0)38 3856187
8281JV Genemuiden Mail info@vebe.net
Netherlands Web www.condor-
group.eu/vebe_floorcoverings
