ENVIRONMENTAL PRODUCT DECLARATION
as per ISO 14025 and EN 15804+A2
Owner of the Declaration Knauf GIps KG
Programme holder Institut Bauen und Umwelt e.V. (IBU)
Publisher Institut Bauen und Umwelt e.V. (IBU)
Declaration number EPD-KNA-20220117-IBA1-EN
Issue date 30.11.2022
Valid to 29.11.2027
Knauf Duralpha F 2202
Knauf Gips KG
www.ibu-epd.com | https://epd-online.com
Umwelt Produktdeklaration Name des Herstellers – Name des Produkts
1. General Information
Knauf Gips KG Knauf Duralpha F 2202
Programme holder Owner of the declaration
IBU – Institut Bauen und Umwelt e.V. Knauf Gips KG
Hegelplatz 1 Am Bahnhof 7
10117 Berlin D-97346 Iphofen
Germany
Declaration number Declared product / declared unit
EPD-KNA-20220117-IBA1-EN 1000 kg Knauf Duralpha F 2202
This declaration is based on the product Scope:
category rules: The EPD applies for Knauf Duralpha F 2202 flowing
Mineral factory-made mortar, 11.2017 screed compound produced in Knauf plant
(PCR checked and approved by the SVR) Niederaußem.
Issue date The owner of the declaration shall be liable for the
30.11.2022 underlying information and evidence; the IBU shall not
be liable with respect to manufacturer information, life
cycle assessment data and evidences.
Valid to
The EPD was created according to the specifications
29.11.2027
of EN 15804+A2. In the following, the standard will be
simplified as EN 15804.
Verification
The standard EN 15804 serves as the core PCR
Independent verification of the declaration and data
according to ISO 14025:2011
Dipl. Ing. Hans Peters internally x externally
(chairman of Institut Bauen und Umwelt e.V.)
Dr. Alexander Röder Matthias Klingler
(Managing Director Institut Bauen und Umwelt e.V.)) (Independent verifier)
2. Product
2.1 Product description/Product definition
2.2 Application
This declaration refers to Knauf Duralpha F 2202
flowing screed compound. Knauf Duralpha F 2202 is Knauf Duralpha F 2202 flowing screed compound is
based on alpha hemihydrate and used for the used to produce calcium sulfate flowing screeds (e.g.,
production of calcium sulfate flowing screed. heated and unheated screed). Those flowing screeds
can be used to install large screed surfaces without
The primary binding agent is represented by bindable joints.
calcium sulfate (alpha hemihydrate) blended with
additives and hydrated as flowing screed by adding 2.3 Technical Data
water and sand.
The following technical properties apply to a flowing
This declaration only applies to the flowing screed screed according to the technical datasheet IC017.de:
compound Knauf Duralpha F 2202 delivered as bulk in
a silo-truck, i.e., not in bags. Constructional data
Name Value Unit
For the placing on the market of the product in the Bulk density 1.12-1.15 kg/dm³
European Union/European Free Trade Association Compressive strength EN 13813 ≥ 25 N/mm2
(EU/EFTA) (with the exception of Switzerland) Flexural strength EN 13813 ≥ 5 N/mm2
Regulation (EU) No. 305/2011 (CPR) applies. The
product needs a declaration of performance taking into
consideration the harmonised standard DIN EN 13454: Performance data of the product in accordance with
Binders, composite binders and factory made mixtures the declaration of performance with respect to its
for floor screeds based on calcium sulfate, DIN EN essential characteristics according to the harmonised
13813: Screed material and floor screeds, and the CE- standard EN 13454-1:2004-09: Binders, composite
marking. binders and factory made mixtures for floor screeds
For the application and use the respective national based on calcium sulfate – Part 1: Definitions and
provisions apply. requirements.
2 Environmental Product Declaration Knauf Gips KG – Knauf Duralpha F 2202
2.4 Delivery status
Knauf Duralpha F 2202 is provided as bulk material for This product contains other carcinogenic, mutagenic,
mobile mixers or truckmixers. reprotoxic (CMR) substances in categories 1A or 1B
(Regulation (EC) No. 1272/2008) which are not on the
2.5 Base materials/Ancillary materials candidate list, exceeding 0.1 percentage by mass: no.
This declaration refers to Knauf Duralpha F 2202
flowing screed compound. It contains binding agents, Biocide products were added to this construction
aggregates as well as additives, whereby aggregates product or it has been treated with biocide products
and additives account for < 3% of the total mass of the (this then concerns a treated product as defined by the
dry mixture. (EU) Ordinance on Biocide Products No. 528/2012):
no.
The main component of Knauf Duralpha F 2202 is
alpha hemihydrate. This compound is mixed with sand
and water on the construction site. The water leads to 2.6 Manufacture
hydration of alpha hemihydrate, which builds the To produce Knauf Duralpha F 2202, Flue gas
flowing screed in combination with the sand with the desulphurization (FGD) gypsum is calcinated to alpha
desired binding capacity. hemihydrate (Figure 1) which is then ground and
mixed with various additives to the final compound.
This product contains substances listed in the
candidate list (date: 2022-06-10, ECHA2022)
exceeding 0.1 percentage by mass: no.
Figure 1: Manufacturing process of alpha hemihydrate
2.10 Condition of use
2.7 Environment and health during Knauf Duralpha F 2202 is an intermediate product to
manufacturing which water and sand are added on the jobsite by
The manufacturing plant in Niederaußem is certified using a mobile mixer. The compound/sand ratio is
according to ISO 45001 and meets the standard to the about 0.5 according to DIN EN 13454-2. The ratio of
Federal Immission Control Act (BImSchG). water to solids is about 0.15.
2.8 Product processing/Installation Calcium sulIfate screeds are typically not suited for
In a mobile mixer, Knauf Duralpha F 2202 is mixed wetrooms. If they are intended for use in wetrooms,
with water and sand to a flowing screed on the jobsite. nevertheless, please refer to the leaflet “Calciumsulfat-
Alternatively, it can be mixed in a concrete plant with Fließestriche in Feuchträumen” (VDPM2022).
sand and water and delivered in a truck mixer as fresh
mortar to the jobsite. It is then pumped to the 2.11 Environment and health during use
respective area where it levels itself. No hazard for humans and the environment is to be
expected if the compound is used as intended.
2.9 Packaging A safety datasheet for Knauf Duralpha F 2202 is
Knauf Duralpha F 2202 is delivered as bulk material in available. SDS2016
a silo-truck. Therefore, no packaging waste is
generated.
3 Environmental Product Declaration Knauf Gips KG – Knauf Duralpha F 2202
2.12 Reference service life desiccate again afterwards. Permanent moisture
The useful life is > 50 years in line with code numbers penetration, on the other hand, can diminish the
352.111 (flowing screeds) or 352.113 (screeds as wear strength of the screeds. That is why those screeds
floors) according to the table “Nutzungsdauern von need to be protected from moisture.
Bauteilen für Lebenszyklusanalysen nach dem
Bewertungssystem Nachhaltiges Bauen (BNB)” Mechanical destruction
(BBSR). Unforeseen mechanical destruction does not result in
environmental damage.
2.13 Extraordinary effects 2.14 Re-use phase
According to the current state of the art, flowing
Fire screeds are not recycled or re-used. Therefore, these
According to DIN 4102-1 Knauf Duralpha F 2202 is screeds are disposed of in landfills.
non-flammable and corresponds with construction
product class A1. 2.15 Disposal
European Waste Code: 17 08 02 gypsum-based
Fire protection construction materials other than those mentioned in
Name Value 17 08 01.
Building material class A1
2.16 Further information
Water Additional information is available at
Temporary moisture penetration will not cause any www.k‑sentials.com.
damage to calcium sulfate screeds if they are able to
3. LCA: Calculation rules
3.1 Declared Unit not declared in the EPD, since they relate to the final
The declared unit is 1000 kg of dry Knauf Duralpha F mixture of flowing screed as installed in the building.
2202 flowing screed compound.
Declared unit 3.3 Estimates and assumptions
Name Value Unit Transport A2:
Declared unit 1000 kg Transport of all additives: truck-trailer, Euro 5, 34-40t
Gross density (average) 1135 kg/m3 gross weight / 27 t payload capacity, capacity
utilization of 50% (including empty runs).
Transport of FGD gypsum via conveyor belt over a
distance of 1 km.
3.2 System boundary
Since Knauf Duralpha F 2202 is mixed with sand and 3.4 Cut-off criteria
water at the building site, the type of EPD "Cradle to Due to small quantities of additives (sum of additives
gate" was chosen. Knauf Duralpha F 2202 cannot be less than 3%) the contributions of their packaging
separated from the installed flowing screed at end of materials to the overall life cycle impacts of the Knauf
life. Therefore, IBU advised to declare modules A1-A3 Duralpha F 2202 are regarded to be very low and are
and C4 with C4 only acounting for the carbon balance therefore not considered in the calculation.
correction of modules A1-A3.
This EPD includes the following modules according to Transports within the manufacturing site have been
DIN EN 15804+A2. neglected due to the short distances and the low
Raw material supply (A1): Knauf Duralpha F 2202 expected environmental impacts resulting from those
consists mainly of alpha hemihydrate and some transports. Further to that, transport losses at the
additives. The alpha hemihydrate is made of FGD manufacturing, e.g., formation of dust at conveyor belts
gypsum, which is a by-product of a nearby lignite-fired as well as the supply and recovery of the raw material
power plant. packaging are not considered.
Transport (A2): Since the FGD gypsum is sourced
from a power plant close to the manufacturing site, a 3.5 Background data
conveyor belt is used for transport. The additives are GaBi was used as LCA software and background
produced in Germany and transported via truck-trailer database (database version 2022.1). Only datasets
to the manufacturing plant. from this software and corresponding database(s)
Manufacturing (A3): Alpha hemihydrate is produced by were used during modelling.
calcining FGD gypsum in an autoclave. Afterwards the
alpha hemihydrate is mixed with additives to Knauf 3.6 Data quality
Duralpha F 2202. Background data provided by the GaBi software
Disposal (C4): This module accounts only for the respective Sphera Solutions GmbH have been
carbon balance correction of the additives that contain updated during the last 5 years.
biogenic carbon. A few additives had to be substituted by processes for
similar functional additives due to missing data in
Transport to the construction site (A4), assembly (A5), GaBi. That is why the overall data quality is evaluated
use stage (B1-B7), de-construction and demolition as satisfactory.
(C1), transport at end-of-life (C2), waste processing
(C3) and reuse-, recovery- recycling potential (D) are
4 Environmental Product Declaration Knauf Gips KG – Knauf Duralpha F 2202
3.7 Period under review No end-of-life modules are declared. Therefore,
For the production data an annual average from the allocations for reuse, recycling and recovery are not
year 2020 was calculated. applicable.
3.8 Allocation 3.9 Comparability
Allocations in the foreground system are avoided as far Basically, a comparison or an evaluation of EPD data
as possible. is only possible if all the data sets to be compared
As there is only one kind of flowing screed compound were created according to EN 15804 and the building
produced at one time in the plant, co-product context, respectively the product-specific
allocations are avoided. Though, in the dataset of FGD characteristics of performance, are taken into account.
gypsum allocations occur. These allocations are
explained in the documentation of the dataset.
4. LCA: Scenarios and additional technical information
Characteristic product properties
Information on biogenic Carbon
Information on describing the biogenic Carbon
Content at factory gate
Name Value Unit
Biogenic Carbon Content in
0.51 kg C
product
Reference service life
Name Value Unit
Life Span (according to BBSR) ≥ 50 a
See section 2.13
5 Environmental Product Declaration Knauf Gips KG – Knauf Duralpha F 2202
5. LCA: Results
DESCRIPTION OF THE SYSTEM BOUNDARY (X = INCLUDED IN LCA; ND = MODULE OR INDICATOR NOT
DECLARED; MNR = MODULE NOT RELEVANT)
BENEFITS AND
CONSTRUCTI LOADS
PRODUCT STAGE ON PROCESS USE STAGE END OF LIFE STAGE BEYOND THE
STAGE SYSTEM
BOUNDARIES
6 Environmental Product Declaration Knauf Gips KG – Knauf Duralpha F 2202
lairetam
waR
ylppus tropsnarT
gnirutcafunaM
eht
morf
tropsnarT
etis
eht
ot
etag
ylbmessA esU
ecnanetniaM
riapeR
tnemecalpeR tnemhsibrufeR
ygrene
lanoitarepO esu
retaw
lanoitarepO esu
noitcurtsnoc-eD
noitilomed tropsnarT
gnissecorp
etsaW
lasopsiD -esueR -yrevoceR -gnilcyceR laitnetop
A1 A2 A3 A4 A5 B1 B2 B3 B4 B5 B6 B7 C1 C2 C3 C4 D
X X X ND ND ND ND MNR MNR MNR ND ND ND ND ND X ND
RESULTS OF THE LCA - ENVIRONMENTAL IMPACT according to EN 15804+A2: 1000 kg Duralpha F 2202
Core Indicator Unit A1-A3 C4
Global warming potential - total [kg CO2-Eq.] 1.77E+2 1.88E+0
Global warming potential - fossil fuels [kg CO2-Eq.] 1.79E+2 0.00E+0
Global warming potential - biogenic [kg CO2-Eq.] -1.66E+0 1.88E+0
GWP from land use and land use change [kg CO2-Eq.] 1.06E-2 0.00E+0
Depletion potential of the stratospheric ozone layer [kg CFC11-Eq.] 1.74E-10 0.00E+0
Acidification potential, accumulated exceedance [mol H+-Eq.] 2.00E-1 0.00E+0
Eutrophication, fraction of nutrients reaching freshwater
[kg P-Eq.] 4.31E-4 0.00E+0
end compartment
Eutrophication, fraction of nutrients reaching marine end
[kg N-Eq.] 5.39E-2 0.00E+0
compartment
Eutrophication, accumulated exceedance [mol N-Eq.] 5.79E-1 0.00E+0
Formation potential of tropospheric ozone photochemical
[kg NMVOC-Eq.] 1.51E-1 0.00E+0
oxidants
Abiotic depletion potential for non-fossil resources [kg Sb-Eq.] 6.07E-6 0.00E+0
Abiotic depletion potential for fossil resources [MJ] 1.67E+3 0.00E+0
Water (user) deprivation potential, deprivation-weighted [m³ world-Eq
7.28E+0 0.00E+0
water consumption (WDP) deprived]
RESULTS OF THE LCA - INDICATORS TO DESCRIBE RESOURCE USE according to EN 15804+A2: 1000
kg Duralpha F 2202
Indicator Unit A1-A3 C4
Renewable primary energy as energy carrier [MJ] 8.10E+1 0.00E+0
Renewable primary energy resources as material utilization [MJ] 3.25E+1 0.00E+0
Total use of renewable primary energy resources [MJ] 1.13E+2 0.00E+0
Non-renewable primary energy as energy carrier [MJ] 1.67E+3 0.00E+0
Non-renewable primary energy as material utilization [MJ] 0.00E+0 0.00E+0
Total use of non-renewable primary energy resources [MJ] 1.67E+3 0.00E+0
Use of secondary material [kg] 0.00E+0 0.00E+0
Use of renewable secondary fuels [MJ] 0.00E+0 0.00E+0
Use of non-renewable secondary fuels [MJ] 0.00E+0 0.00E+0
Use of net fresh water [m³] 4.48E-1 0.00E+0
RESULTS OF THE LCA – WASTE CATEGORIES AND OUTPUT FLOWS according to EN 15804+A2:
1000 kg Duralpha F 2202
Indicator Unit A1-A3 C4
Hazardous waste disposed [kg] 2.36E-8 0.00E+0
Non-hazardous waste disposed [kg] 1.28E+0 0.00E+0
Radioactive waste disposed [kg] 3.72E-2 0.00E+0
Components for re-use [kg] 0.00E+0 0.00E+0
Materials for recycling [kg] 0.00E+0 0.00E+0
Materials for energy recovery [kg] 0.00E+0 0.00E+0
Exported electrical energy [MJ] 0.00E+0 0.00E+0
Exported thermal energy [MJ] 0.00E+0 0.00E+0
RESULTS OF THE LCA – additional impact categories according to EN 15804+A2-optional:
1000 kg Duralpha F 2202
Indicator Unit A1-A3 C4
Potential incidence of disease due to PM emissions [Disease
1.56E-6 0.00E+0
Incidence]
Potential Human exposure efficiency relative to U235 [kBq U235-
2.65E+0 0.00E+0
Eq.]
Potential comparative toxic unit for ecosystems [CTUe] 4.30E+2 0.00E+0
Potential comparative toxic unit for humans - cancerogenic [CTUh] 9.90E-9 0.00E+0
Potential comparative toxic unit for humans - not cancerogenic [CTUh] 1.09E-6 0.00E+0
Potential soil quality index [-] 2.34E+2 0.00E+0
Disclaimer 1 – for the indicator “Potential Human exposure efficiency relative to U235”. This impact category
deals mainly with the eventual impact of low dose ionizing radiation on human health of the nuclear fuel cycle. It
does not consider effects due to possible nuclear accidents, occupational exposure or radioactive waste disposal
in underground facilities. Potential ionizing radiation from the soil, radon and from some construction materials is
also not measured by this indicator.
Disclaimer 2 – for the indicators “abiotic depletion potential for non-fossil resources”, “abiotic depletion potential
for fossil resources”, “water (user) deprivation potential, deprivation-weighted water consumption”, “potential
comparative toxic unit for ecosystems”, “potential comparative toxic unit for humans – cancerogenic”, “Potential
comparative toxic unit for humans - not cancerogenic”, “potential soil quality index”. The results of this
environmental impact indicator shall be used with care as the uncertainties on these results are high as there is
limited experience with the indicator.
Disclaimer 3 - as already mentioned in 3.2 System Boundary as advice from IBU only the modules A1-A3 and C4
are declared whereby C4 is only for carbon balance correction of the modules A1-A3
6. LCA: Interpretation
Production significantly dominates the LCA impact energy sources. This process is responsible for more
categories due to the calcination of the FGD gypsum at than 80% of the GWP.
about 180°C associated with the consumption of fossil Module C4 is only declared to account for the carbon
balance correction of modules A1-A3.
7. Requisite evidence
0.3 mSv/a, determined on the basis of the index
7.1 Leaching calculation to RP 112 and the radon concentration BfS
On analysis according to the Landfilling Ordinance, report.
Knauf Duralpha F 2202 displays the sulfate
concentration in the saturation range which is typical 7.3 VOC emissions
for gypsum (approx. 1500 mg/l), resulting in disposal The requirement in accordance with the AgBB test
options only from landfill class I upwards. Gypsum is scheme (version 2018) were confirmed by
classified as a listed substance in Water Hazard Class Servaco/Normec Product Testing.
1 (slightly hazardous for water). Heavy metal content is After 3 days:
significantly lower than the allocation criteria for TVOC: ≤ 10 mg/m³
landfilling class I. The waste producer is responsible Carcinogens EU cat. 1 and 2: ≤ 0.01 mg/m³
for the proper disposal. Proper disposal depends on After 28 days
parameters like use, sorting depth during de- TVOC: < 1.0 mg/m³
construction, collection (separately or together with SVOC: ≤ 0.1 mg/m³
other construction waste) and treatment. Sum Ri: < 1
TVOC excl. LCI: ≤ 0.1 mg/m³
7.2 Radioactivity Carcinogens EU cat. 1 and 2: ≤ 0.001 mg/m³
The product can be used without restriction with overall Formaldehyde: ≤ 0.12 mg/m³
dose contributions of significantly lower than
8. References
Standards
DIN 4102-1 EN 15804
DIN 4102-1:1998-05, Fire behaviour of building EN 15804:2019+A2+AC:2021, Sustainability of
materials and building components - Part 1: Building construction works — Environmental Product
materials; concepts, requirements and tests Declarations — Core rules for the product category of
construction products.
DIN EN 13454
DIN EN 13454-1:2005-01, Binders, composite binders ISO 14025
and factory made mixtures for floor screeds based on DIN EN ISO 14025:2011-10, Environmental labels and
calcium sulfate - Part 1: Definitions and requirements declarations — Type III environmental declarations —
Principles and procedures.
EN 13501
EN 13501-1: 2018, Fire classification of construction ISO 14040
products and building elements - Part 1: Classification ISO 14040:2006 + Amd 1:2020, Environmental
using data from reaction to fire tests management – Life cycle assessment – Principles and
framework; English version EN ISO 14040:2006 +
EN 13813 A1:2020, English translation of DIN EN ISO
DIN EN 13813:2003-01, Screed material and floor 14040:2021-02
screeds - Screed materials - Properties and
requirements ISO 14044
7 Environmental Product Declaration Knauf Gips KG – Knauf Duralpha F 2202
ISO 14044:2006 + Amd 1:2017 + Amd 2:2020, Bau- und Abbruchabfällen (Gewerbeabfallverordnung -
Environmental management – Life cycle assessment – GewAbfV) Gewerbeabfallverordnung vom 18. April
Requirements and guidelines; English version EN ISO 2017 (BGBl. I S. 896), last amended by Artikel 3 der
14044:2006 + A1:2018 + A2:2020, English translation Verordnung vom 28. April 2022 (BGBl. I S. 700)
of DIN EN ISO 14044:2021-02 German Commercial Waste Ordinance
ISO 15686 IBU PCR Part A
ISO 15686-2:2012-05, Buildings and constructed Institut Bauen und Umwelt e.V.: Product Category
assets - Service life planning - Part 2: Service life Rules for Building-Related Products and Services Part
prediction procedures A: Calculation Rules for the Life Cycle Assessment
and Requirements on the Project Report according to
ISO 45001 EN 15804+A2:2019, v1.1.2, 2021-09-02
DIN ISO 45001:2018-06: Occupational health and
safety management systems - Requirements with IBU PCR Part B "Mineral factory-made mortar"
guidance for use Institut Bauen und Umwelt e.V.: PCR Guidance-Texts
for Building-Related Products and Services Part B:
Further References Requirements on the EPD for Mineral factory-made
AgBB mortar, v1.6, 2017-11-30
AgBB - Evaluation procedure for VOC emissions from
building products, Committee for Health-related IC017.de
Evaluation of Building Products, 2018 Product Data Sheet Knauf K-Sentials Duralpha F
2202, Knauf Gips KG, Iphofen, 2020-03
BBSR (IC017.de/eng/03.20/0/TB)
Service life of building components for life cycle
analyses according to the Assessment System for Landfilling Ordinance
Sustainable Building, editor: German Federal Institute Verordnung über Deponien und Langzeitlager
for Research on Building, Urban Affairs and Spatial (Deponieverordnung - DepV), Deponieverordnung vom
Development, 2017 (Nutzungsdauern von Bauteilen für 27. April 2009 (BGBl. I S. 900), Zuletzt geändert durch
Lebenszyklusanalysen nach Bewertungssystem Art. 3 V v. 9.7.2021 I 2598
Nachhaltiges Bauen (BNB), Bundesinstitut für Bau-,
Stadt- und Raumforschung (BBSR), Stand 24.02.2017) VDPM2022
Merkblatt 1: Calciumsulfat-Fließestriche in
BfS report Feuchträumen - Hinweise und Richtlinien für die
K. Gehrcke, B. Hoffmann, U. Schade, V. Schmidt, K. Planung und Ausführung von Calciumsulfat-
Wichterey: Natürliche Radioaktivität in Baumaterialien Fließestrichen (Flowing calcium sulphate screeds in
und die daraus resultierende Strahlenexposition areas of high humidity), Verband für Dämmsysteme,
(Natural radioactivity in construction materials and the Putz und Mörtel e. V. und der Industriegruppe
ensuing radiation exposure), Federal Office for Estrichstoffe im Bundesverband der Gipsindustrie e.
Radiation Protection, Salzgitter, November 2012 V., Berlin, 2022
ECHA 2022 (EU) Ordinance on Biocide Products No. 528/2012
European Chemicals Agency (ECHA), Candidate List REGULATION (EU) No 528/2012 OF THE
of Substances of Very High Concern for Authorisation EUROPEAN PARLIAMENT AND OF THE COUNCIL
(published in accordance with Article 59(10) of the of 22 May 2012 concerning the making available on
REACH Regulation) the market and use of biocidal products
http://echa.europa.eu/de/candidate-list-table ,
Revision: 2022-06-10. Regulation (EU) No. 305/2011
REGULATION (EU) No 305/2011 OF THE
European Waste Code EUROPEAN PARLIAMENT AND OF THE COUNCIL
Guidance on classification of waste according to EWC- of 9 March 2011 laying down harmonised conditions
Stat categories, Supplement to the Manual for the for the marketing of construction products and
Implementation of the Regulation (EC) No 2150/2002 repealing Council Directive 89/106/EEC
on Waste Statistics, COMMISSION OF THE
EUROPEAN COMMUNITIES/EUROSTAT, v2, Regulation (EC) No. 1272/2008
December 2010 REGULATION (EC) No 1272/2008 OF THE
EUROPEAN PARLIAMENT AND OF THE COUNCIL
Federal Immission Control Act (BImSchG) of 16 December 2008 on classification, labelling and
Federal Immission Control Act (Bundes- packaging of substances and mixtures, amending and
Immisionsschutzgesetz, BImSchG), last amended by repealing Directives 67/548/EEC and 1999/45/EC, and
Article 1 of the Act of 3 May 2000 (Federal Law amending Regulation (EC) No 1907/2006
Gazette I. p. 632)
RP 112
GaBi Radiation Protection 112 - Radiological protection
GaBi ts (v10.6.1.35): Software-System and Databases principles concerning the natural radioactivity of
for Life Cycle Engineering, Sphera Solutions GmbH, building materials, European Commission, 1999
Leinfelden-Echterdingen, Germany, 2022 (database
version 2022.1) SDS2016
Safety data sheet “Duralpha F 2003, Duralpha F 2201,
GewAbfV Duralpha F2202”, Knauf Gips KG, Iphofen, 2016-01-28
Verordnung über die Bewirtschaftung von
gewerblichen Siedlungsabfällen und von bestimmten
8 Environmental Product Declaration Knauf Gips KG – Knauf Duralpha F 2202
9 Environmental Product Declaration Knauf Gips KG – Knauf Duralpha F 2202
Publisher
Institut Bauen und Umwelt e.V. Tel +49 (0)30 3087748- 0
Hegelplatz 1 Fax +49 (0)30 3087748- 29
10117 Berlin Mail info@ibu-epd.com
Germany Web www.ibu-epd.com
Programme holder
Institut Bauen und Umwelt e.V. Tel +49 (0)30 - 3087748- 0
Hegelplatz 1 Fax +49 (0)30 – 3087748 - 29
10117 Berlin Mail info@ibu-epd.com
Germany Web www.ibu-epd.com
Author of the Life Cycle
Assessment Tel 0049 9001 31-1000 *
Knauf Gips KG Fax 0049 1805 31-4000 *
Am Bahnhof 7 Mail knauf-direkt@knauf.de
97346 Iphofen Web www.knauf.de
Germany
Owner of the Declaration
Knauf Gips KG Tel 0049 9001 31-1000 *
Am Bahnhof 7 Fax 0049 1805 31-4000 *
97346 Iphofen Mail knauf-direkt@knauf.de
Germany Web www.knauf.de
