ENVIRONMENTAL PRODUCT DECLARATION
as per ISO 14025 and EN 15804+A2
Owner of the Declaration dormakaba International Holding GmbH
Publisher Institut Bauen und Umwelt e.V. (IBU)
Programme holder Institut Bauen und Umwelt e.V. (IBU)
Declaration number EPD-DOR-20220215-CBA1-EN
Issue date 19.10.2022
Valid to 18.10.2027
TS 92 XEA
dormakaba
www.ibu-epd.com | https://epd-online.com
General Information
dormakaba TS 92 XEA
Programme holder Owner of the declaration
IBU – Institut Bauen und Umwelt e.V. dormakaba International Holding GmbH
Hegelplatz 1 DORMA Platz 1
10117 Berlin 58256 Ennepetal
Germany Germany
Declaration number Declared product / declared unit
EPD-DOR-20220215-CBA1-EN 1 door closer (1 piece) of the TS 92 XEA
This declaration is based on the product category rules: Scope:
Building Hardware products, 01.08.2021 This Environmental Product Declaration refers to a specific door closer
(PCR checked and approved by the SVR) manufactured by dormakaba Production GmbH & CO KG. The production
site is located in Singapore.
Issue date The data represents the year 2020.
The owner of the declaration shall be liable for the underlying information
19.10.2022
and evidence; the IBU shall not be liable with respect to manufacturer
information, life cycle assessment data and evidences.
Valid to
The EPD was created according to the specifications of EN 15804+A2. In
18.10.2027 the following, the standard will be simplified as EN 15804.
Verification
The standard EN 15804 serves as the core PCR
Independent verification of the declaration and data according to ISO
14025:2011
internally X externally
Dipl.-Ing. Hans Peters
(Chairman of Institut Bauen und Umwelt e.V.)
Florian Pronold Dr.-Ing. Wolfram Trinius,
(Managing Director Institut Bauen und Umwelt e.V.) (Independent verifier)
1 Environmental Product Declaration - dormakaba - TS 92 XEA
Product
Product description/Product definition Base materials/Ancillary materials
The universal slide channel door closer for standard doors The major material compositions including the packaging of the
features EASY OPEN technology for easy door opening. The product are listed below:
TS 92 XEA slide channel door closer is an attractive and Name Value Unit
competitively priced complement to the TS 98 XEA range. The
Steel 38 %
XEA design ensures a uniform appearance in the complete
Aluminium 37 %
building. For the use and application of the product the
respective national provisions at the place of use apply. The Paper 14 %
standards which can be applied are the following: Zinc 4 %
• EN 1154 Lubricants 4 %
• EN 1634-1 Plastics 2 %
Others 1 %
Application
It can be used for any interior application. The product includes partial articles which contain substances
listed in the Candidate List of REACH Regulation
Technical Data 1907/2006/EC (date: 17.01.2022) exceeding 0.1 percentage by
The door closer has following technical properties: mass: yes
• Lead (Pb): 7439-92-1 (CAS-No.) is included in some of
the alloys used. The concentration of lead in each
individual alloy does not exceed 4.0% (by mass).
The Candidate List can be found on the ECHA website
address: https:echa.europa.eu/de/home.
Reference service life
The reference service life of the TS 92 XEA door closer
depends on the traffic pattern and degree of usage of the door.
These closers are rated to EN 1154, meaning they are
designed to withstand a minimum of 500,000 cycles. The
reference service life amounts for 20 years. This corresponds
with approx. 25,000 cycles per year.
Performance data of the product with respect to its
characteristics in accordance with the relevant technical
provision which can be applied are mentioned above.
LCA: Calculation rules
Construction stage - Modules A4-A5
Declared Unit The construction process stage includes:
The declared unit is 1 piece of the product: TS 92 XEA. — A4, transport to the building site;
Declared unit — A5, installation into the building;
including provision of all materials, products and energy, as well
Name Value Unit
as waste processing up to the end-of waste state or disposal of
Declared unit 1 piece/product
final residues during the construction process stage.
Conversion factor to 1 kg kg per declared
0.29 -
product End-of-life stage– Modules C1-C4 and D
Mass of declared Product 3.34 kg The end-of-life stage includes:
— C1, de-construction, demolition:
System boundary — C2, transport to waste processing;
— C3, waste processing for reuse, recovery and/or recycling;
The type of EPD is: cradle to gate with options, modules C1–
— C4, disposal;
C4, and module D (A1–A3 + C + D and additional modules: A4
including provision and all transport, provision of all materials,
+ A5)
products and related energy and water use.
Production - Module A1-A3
Module D (Benefits and loads beyond the system boundary)
The product stage includes:
includes:
— A1, raw material extraction, processing and mechanical
— D, recycling potentials, expressed as net impacts and
treatments, processing of secondary material input (e.g.
benefits.
recycling processes), — A2, transport to the manufacturer,
— A3, manufacturing and assembly including provision of all
Geographic Representativeness
materials, products and energy, as well as waste processing up
Land or region, in which the declared product system is
to the end-of waste state.
manufactured, used or handled at the end of the product´s
lifespan: Singapore
2 Environmental Product Declaration - dormakaba - TS 92 XEA
Comparability
Basically, a comparison or an evaluation of EPD data is only
possible if all the data sets to be compared were created
according to EN 15804 and the building context, respectively
the product-specific characteristics of performance, are taken
into account.
LCA: Scenarios and additional technical information
End of life (C1-C4)
Characteristic product properties of biogenic carbon
C1: The product dismantling from the building is done manually
Information on describing the biogenic Carbon Content at without environmental burden.
factory gate C2: Transport to waste treatment at end of life is 50 km.
Name ValueUnit Name Value Unit
Biogenic carbon content in product 0.15 kg Collected separately waste type waste type 3.28 kg
C
Recycling 3.22 kg
Biogenic carbon content in accompanying kg
0.02 Energy recovery 0.059 kg
packaging C
Final disposal 0,13 kg
Note: 1 kg of biogenic carbon is equivalent to 44/12 kg of CO .
2
Reuse, recovery and/or recycling potentials (D), relevant
scenario information
Additional technical information for the declared modules. Name Value Unit
Transport to the building site (A4) Recycling 100 %
Name Value Unit Collection rate is 100%.
Litres of fuel truck (per piece) 0.00276l/100km
Transport distance via truck (from habor to
300 km
dormakaba logistic center)
Transport distance via truck (for scaling) 100 km
Capacity utilisation (including empty runs)
55 %
average
Transport distance via ship 11000 km
The product is transported via truck and ship. The product is
stored in the dormakaba logistic center in Germany. The main
distribution region is Europe. In order to allow scaling to a
specific point of installation 100 km are declared as well.
Installation into the building (A5)
Name ValueUnit
Output substances following waste treatment on
0.06 kg
site (packaging)
3 Environmental Product Declaration - dormakaba - TS 92 XEA
LCA: Results
DESCRIPTION OF THE SYSTEM BOUNDARY (X = INCLUDED IN LCA; MND = MODULE OR INDICATOR NOT DECLARED; MNR
= MODULE NOT RELEVANT)
Benefits and
Construction loads beyond
Product stage Use stage End of life stage
process stage the system
boundaries
la ire ta m w a Ry lp p u s tro p s n a rT g n iru tc a fu n a M e h t m o rf tro p s n a rTe tis e h t o t e ta g y lb m e s s A e s U e c n a n e tn ia M ria p e R tn e m e c a lp e R tn e m h s ib ru fe R y g re n e la n o ita re p Oe s u re ta w la n o ita re p Oe s u n o itc u rts n o c -e Dn o itilo m e d tro p s n a rT g n is s e c o rp e ts a W la s o p s iD -e s u e R-y re v o c e R-g n ilc y c e Rla itn e to p
A1 A2 A3 A4 A5 B1 B2 B3 B4 B5 B6 B7 C1 C2 C3 C4 D
X X X X X MND MND MNR MNR MNR MND MND X X X X X
RESULTS OF THE LCA - ENVIRONMENTAL IMPACT according to EN 15804+A2: 1 door closer
Parameter Unit A1-A3 A4 A5 C1 C2 C3 C4 D
GWP-total kg CO 2 eq 2.52E+01 2.37E-01 8.5E-02 0 1.4E-02 1.29E+00 0 -9.03E+00
GWP-fossil kg CO 2 eq 2.59E+01 2.32E-01 2E-03 0 1.4E-02 5.62E-01 0 -9E+00
GWP-biogenic kg CO 2 eq -7.44E-01 5E-03 8.3E-02 0 6.32E-04 7.31E-01 0 -2.8E-02
GWP-luluc kg CO 2 eq 9E-03 5.13E-06 1.4E-06 0 3.25E-07 3.83E-05 0 -2E-03
ODP kg CFC11 eq 8.97E-11 2.31E-17 1.53E-17 0 1.44E-18 3.68E-16 0 -6.19E-11
AP mol H+ eq 1.29E-01 5E-03 2.38E-05 0 1.37E-05 2.04E-04 0 -3.3E-02
EP-freshwater kg P eq 2.48E-05 5.1E-08 3E-09 0 2.93E-09 5.78E-08 0 -5.87E-06
EP-marine kg N eq 2.06E-02 1E-03 8.6E-06 0 4.35E-06 5.67E-05 0 -4E-03
EP-terrestrial mol N eq 2.19E-01 1.3E-02 1.07E-04 0 4.84E-05 9.48E-04 0 -4.8E-02
kg NMVOC
POCP 6.3E-02 3E-03 2.28E-05 0 1.23E-05 1.55E-04 0 -1.4E-02
eq
ADPE kg Sb eq 6.16E-04 6.44E-09 2.42E-10 0 4.1E-10 5.25E-09 0 -1.93E-04
ADPF MJ 2.81E+02 3.04E+00 2.7E-02 0 1.94E-01 4.15E-01 0 -1.27E+02
m3 world eq
WDP 3.9E+00 4.35E-04 1.1E-02 0 2.68E-05 1.33E-01 0 -5.04E-01
deprived
GWP = Global warming potential; ODP = Depletion potential of the stratospheric ozone layer; AP = Acidification potential of land and water; EP =
Eutrophication potential; POCP = Formation potential of tropospheric ozone photochemical oxidants; ADPE = Abiotic depletion potential for non-fossil
resources; ADPF = Abiotic depletion potential for fossil resources; WDP = Water (user) deprivation potential)
RESULTS OF THE LCA - INDICATORS TO DESCRIBE RESOURCE USE according to EN 15804+A2: 1 door closer
Parameter Unit A1-A3 A4 A5 C1 C2 C3 C4 D
PERE MJ 5.39E+01 1E-02 7.25E-01 0 6.11E-04 4.99E+00 0 -5.49E+01
PERM MJ 5.61E+00 0 -7.2E-01 0 0 -4.89E+00 0 0
PERT MJ 5.95E+01 1E-02 5E-03 0 6.11E-04 9.6E-02 0 -5.49E+01
PENRE MJ 2.79E+02 3.04E+00 2.7E-02 0 1.94E-01 2.43E+00 0 -1.27E+02
PENRM MJ 2.02E+00 0 0 0 0 -2.02E+00 0 0
PENRT MJ 2.81E+02 3.04E+00 2.7E-02 0 1.94E-01 4.15E-01 0 -1.27E+02
SM kg 9.8E-01 0 0 0 0 0 0 0
RSF MJ 0 0 0 0 0 0 0 0
NRSF MJ 0 0 0 0 0 0 0 0
FW m3 1.48E-01 1.76E-05 2.48E-04 0 1.1E-06 3E-03 0 -9.7E-02
PERE = Use of renewable primary energy excluding renewable primary energy resources used as raw materials; PERM = Use of renewable primary
energy resources used as raw materials; PERT = Total use of renewable primary energy resources; PENRE = Use of non-renewable primary energy
excluding non-renewable primary energy resources used as raw materials; PENRM = Use of non-renewable primary energy resources used as raw
materials; PENRT = Total use of non-renewable primary energy resources; SM = Use of secondary material; RSF = Use of renewable secondary fuels;
NRSF = Use of non-renewable secondary fuels; FW = Use of net fresh water
RESULTS OF THE LCA – WASTE CATEGORIES AND OUTPUT FLOWS according to EN 15804+A2:
1 door closer
Parameter Unit A1-A3 A4 A5 C1 C2 C3 C4 D
HWD kg 3.42E-06 2.97E-10 3.96E-11 0 1.88E-11 1.09E-09 0 -9.5E-07
NHWD kg 4.26E+00 3.11E-04 3E-03 0 1.98E-05 6.3E-02 0 -1.99E+00
RWD kg 6.74E-03 3.32E-06 1.41E-06 0 2.08E-07 1.86E-05 0 -1.3E-02
CRU kg 0 0 0 0 0 0 0 0
MFR kg 0 0 0 0 0 2.65E+00 0 0
MER kg 0 0 0 0 0 0 0 0
EEE MJ 0 0 1.29E-01 0 0 0 0 0
EET MJ 0 0 2.33E-01 0 0 0 0 0
HWD = Hazardous waste disposed; NHWD = Non-hazardous waste disposed; RWD = Radioactive waste disposed; CRU = Components for re-use;
MFR = Materials for recycling; MER = Materials for energy recovery; EEE = Exported electrical energy; EET = Exported thermal energy
4 Environmental Product Declaration - dormakaba - TS 92 XEA
RESULTS OF THE LCA – additional impact categories according to EN 15804+A2-optional:
1 door closer
Parameter Unit A1-A3 A4 A5 C1 C2 C3 C4 D
Disease
PM 3.13E-06 7.62E-08 1.32E-10 0 7.19E-11 1.79E-09 0 -5.18E-07
incidence
IR kBq U235 eq 1.05E+00 4.77E-04 2.18E-04 0 2.98E-05 2E-03 0 -2.63E+00
ETP-fw CTUe 9.59E+01 2.15E+00 1.3E-02 0 1.37E-01 1.65E-01 0 -4.53E+01
HTP-c CTUh 1.22E-08 4.05E-11 6.74E-13 0 2.58E-12 1.29E-11 0 -1.65E-10
HTP-nc CTUh 3.5E-07 1.82E-09 2.92E-11 0 1.11E-10 1E-09 0 1.36E-07
SQP SQP 1.07E+02 8E-03 7E-03 0 4.98E-04 1.21E-01 0 -4.35E+00
PM = Potential incidence of disease due to PM emissions; IR = Potential Human exposure efficiency relative to U235; ETP-fw = Potential comparative
Toxic Unit for ecosystems; HTP-c = Potential comparative Toxic Unit for humans (cancerogenic); HTP-nc = Potential comparative Toxic Unit for humans
(not cancerogenic); SQP = Potential soil quality index
Disclaimer 1 – for the indicator “Potential Human exposure efficiency relative to U235”. This impact category deals mainly with the
eventual impact of low-dose ionizing radiation on human health of the nuclear fuel cycle. It does not consider effects due to possible
nuclear accidents, occupational exposure or radioactive waste disposal in underground facilities. Potential ionizing radiation from the
soil, radon and from some construction materials is also not measured by this indicator.
Disclaimer 2 – for the indicators “abiotic depletion potential for non-fossil resources”, “abiotic depletion potential for fossil resources”,
“water (user) deprivation potential, deprivation-weighted water consumption”, “potential comparative toxic unit for ecosystems”,
“potential comparative toxic unit for humans – cancerogenic”, “Potential comparative toxic unit for humans - not cancerogenic”,
“potential soil quality index”. The results of this environmental impact indicator shall be used with care as the uncertainties on these
results are high as there is limited experience with the indicator.
References
EN 1154 GaBi
EN 1154-2003; Building hardware - Controlled door closing Sphera Solutions GmbH Gabi Software System and Database
devices - Requirements and test methods for Life Cycle Engineering 1992-2020 Version 10.0.0.71
University of Stuttgart Leinfelden-Echterdingen
EN 1634-1
EN 1634-1:2018; Fire resistance and smoke control tests for GaBi ts documentation
door and shutter assemblies, openable windows and elements GaBi life cycle inventory data documentation (https://www.gabi-
of building hardware - Part 1: Fire resistance test for door and software.com/support/gabi/gabidatabase- 2020-lci-
shutter assemblies and openable windows documentation/).
ISO 14025 LCA-tool dormakabaLCA-tool, IBU-DOR-202104-LT1-EN,
DIN EN ISO 14025:2011-10, Environmental labels and 2021,developed by Sphera Solutions GmbH
declarations — Type III environmental declarations —
Principles and procedures PCR Part A
PCR – Part A: Calculation Rules for the Life Cycle Assessment
EN 15804 and Requirements on the Project Re-port according to EN
EN 15804+A2:2019+AC:2021, Sustainability of construction 15804+A2:2019, Version 1.0, 2020, Institut Bauen und Umwelt
works — Environmental Product Declarations — Core rules for e.V., www.ibu-epd.com
the product category of construction products
PCR Part B
REACH Regulation PCR – Part B: Requirements on the EPD for Building Hardware
Regulation (EC) No 1907/2006 of the European Parliament and product, version 1.2, Institut Bauen und Umwelt e.V., www.ibu-
of the Council on the Registration, Evaluation, Authorisation epd.com, 2017
and Restriction of Chemicals (REACH)
Further References
IBU
Institut Bauen und Umwelt e.V.: General Programme
Instructions for the Preparation of EPDs at the Institut Bauen
und Umwelt e.V. Version 1., Berlin: Institut Bauen und Umwelt
e.V., 2016. www.ibu-epd.com
5 Environmental Product Declaration - dormakaba - TS 92 XEA
Publisher
Institut Bauen und Umwelt e.V. +49 (0)30 3087748- 0
Hegelplatz 1 info@ibu-epd.com
10117 Berlin www.ibu-epd.com
Germany
Programme holder
Institut Bauen und Umwelt e.V. +49 (0)30 3087748- 0
Hegelplatz 1 info@ibu-epd.com
10117 Berlin www.ibu-epd.com
Germany
Author of the Life Cycle Assessment
Sphera Solutions GmbH +49 711 341817-0
Hauptstraße 111- 113 info@sphera.com
70771 Leinfelden-Echterdingen www.sphera.com
Germany
Owner of the Declaration
dormakaba International Holding GmbH +49 2333 793-0
DORMA Platz 1 info.de@dormakaba.com
58256 Ennepetal www.dormakaba.com
Germany
6 Environmental Product Declaration - dormakaba - TS 92 XEA
