ENVIRONMENTAL PRODUCT DECLARATION
as per ISO 14025 and EN 15804+A2
Owner of the Declaration France Metal Steel Doors & Frames
Programme holder Institut Bauen und Umwelt e.V. (IBU)
Publisher Institut Bauen und Umwelt e.V. (IBU)
Declaration number EPD-FRM-20210160-CBA1-EN
Issue date 05.01.2022
Valid to 04.01.2027
Medallion Steel Door
France Metal Steel Doors & Frames
www.ibu-epd.com | https://epd-online.com
Umwelt Produktdeklaration Name des Herstellers – Name des Produkts
General Information
France Metal Medallion Steel Door
Programme holder Owner of the declaration
IBU – Institut Bauen und Umwelt e.V. French Company for Metallic Industries (France Metal)
Panoramastr. 1 9A Shafik Ghorbal St., Roxy
10178 Berlin 11341 Cairo
Germany Egypt
Declaration number Declared product / declared unit
EPD-FRM-20210160-CBA1-EN the Declaration represent 1 Hollow Metal Medallion
Door with Steel Stiffened Core which consists of the
following items:
- Steel Frame
- Medallion Door leaf
This declaration is based on the product Scope:
category rules: This EPD specifies the environmental impacts of 1 unit
Windows and doors , 01.2019 of Hollow Metal Medallion Door with Steel Stiffened
(PCR checked and approved by the SVR) Core with packaging.
This declaration is relevant to the product
Issue date manufactured in France Metal's Factory at 10th of
Ramadan, Egypt.
05.01.2022
Valid to The owner of the declaration shall be liable for the
underlying information and evidence; the IBU shall not
04.01.2027
be liable with respect to manufacturer information, life
cycle assessment data and evidences.
The EPD was created according to the specifications
of EN 15804+A2. In the following, the standard will be
simplified as EN 15804.
Verification
The standard EN 15804 serves as the core PCR
Independent verification of the declaration and data
according to ISO 14025:2010
Dipl. Ing. Hans Peters internally x externally
(chairman of Institut Bauen und Umwelt e.V.)
Dr. Alexander Röder Dr. Stefan Diederichs
(Managing Director Institut Bauen und Umwelt e.V.)) (Independent verifier)
Product
Product description/Product definition  BS 476 part 22
Product Name: Medallion Steel Door  ASTM E90
This Declaration represents a specific 0.91 m × 2.1 m
 ASTM E283
× 0.04 m thick steel door manufactured in France
Metal, Egypt.
 Singles and pairs, available in stainless steel For the placing on the market of the product in the
 optional sound ratings available European Union/European Free Trade Association
(EU/EFTA) (with the exception of Switzerland)
 Bullet resistant ratings available
Regulation (EU) No. 305/2011 (CPR) applies. The
 Polyester powder paint finish product needs a declaration of performance taking into
 Fire ratings up to 240 minutes consideration EN 16034:2014, Pedestrian doorsets,
 Blast resistant ratings up to 100+ PSI industrial, commercial, garage doors and openable
windows. Product standard, performance
 vision lights within doors
characteristics. Fire resisting and/or smoke control
 Sidelights, Transoms and borrowed lights
characteristics and the CE-marking. For the application
 Air infiltration</= 0,10 CFM/sq.ft and use the respective national provisions apply.
Application
the Standards that can be applied for France Metal's The product can be used at interior or exterior in
Medallion steel door are: Commercial buildings such as schools/training centres,
institutional facilities, government buildings,
 ANSI/UL10B , UL10C
2 Environmental Product Declaration France Metal – Medallion Door
warehouses/factories, manufacturing plants,
transportation terminals, etc. Base materials/Ancillary materials
Technical Data The composition of medallion steel doors is as follows :
For the declared product, the following technical data
in the delivery status must be provided with reference Name Value Unit
to the test standard: Steel (Steel sheet and parts) 94 %
Core (Rockwool core) 4 %
Technical Data Other (Glue, Packaging) 2 %
Name Value Unit
Airborne sound reduction ,Rw,(c,ctr), 1) This product/article/at least one partial article
42 dB
optional contains substances listed in the candidate list (date:
Fire resistance class (for fire windows 240 23.04.2021) exceeding 0.1 percentage by mass: NO.
class
and doors) DIN EN 1634-1 minutes
Installation depth 150 mm 2) This product/article/at least one partial article
Fire or contains other carcinogenic, mutagenic, reprotoxic
smoke (CMR) substances in categories 1A or 1B which are
protectio not on the candidate list, exceeding 0.1 percentage by
Possible opening types n, - mass: NO.
Emerge
ncy Exit 3) Biocide products were added to this construction
doors product or it has been treated with biocide products
Steel (this then concerns a treated product as defined by the
Material used (door frame) -
sheets (EU) Ordinance on Biocide Products No. 528/2012):
NO.
(CE-marking according to EN 16034:2014)
Reference service life
The reference service life (RSL) is not declared. A
calculation according to ISO 15686 is not applied. A
Performance data of the product in accordance with
service life of 30 years is declared based on the
the declaration of performance with respect to its
manufacturer’s declaration.
essential characteristics according to EN 16034:2014,
EN 16034:2014, Pedestrian door sets, industrial,
commercial, garage doors and openable windows.
Product standard, performance characteristics. Fire
resisting and/or smoke control characteristics.
LCA: Calculation rules
Declared Unit etc.) used in manufacturing the product. Transportation
The Declaration refers to the functional unit of 1 unit of of these raw materials and energy consumption from
France Metal's Medallion Door with frame. electricity and light fuel oil within the manufacturing
plant are considered in the scope of this module.
Declared unit
Name Value Unit A4 – Transport to installation site: Average distance
with a of 1000 km considered for the transport from the
dimension manufacturing plant to various construction sites.
Declared unit (Specific dimension) 1 0.91 m ×
2.1 m × A5 – Installation: Packaging waste processing.
0.04 m
conversion factor [Mass/Declared End-of-life:
- -
Unit]
Mass of the Product (including C1 – Dismantling/Demolition: No impact as the
75.086 kg
packaging) dismantling could be manual.
Mass of the product (excluding
73.046 kg
packaging weight) C2 – Transport to treatment/disposal site: Average
Conversion factor to 1 kg 73.046 - transport distance of 50 km from the demolition site to
Declared unit 1 pce. waste treatment (recycling) site.
It is a specific EPD with cradle to gate with options C3 – Waste processing (recycling): No impacts from
(A4-A5), modules C1–C4, and module D (A1–A3 + C + waste processing for recycling.
D and additional modules
C4 – Disposal: Landfill of part of steel and other
product components.
System boundary
The following Life Cycle Stages were considered: Benefits and loads beyond the product system
boundary (D): The potential benefits from packaging
Production (A1-A3): Extraction and manufacturing of material are declared. For waste incineration
all supply materials (steel sheets, glue, rubber, paint combustion in a waste incineration plant (R1 > 0.6)
3 Environmental Product Declaration France Metal – Medallion Door
with energy recuperation is considered. The benefits In the assessment, all available data from the
and loads from steel recycling are considered under production process are considered, i.e. all raw
module D. materials used, auxiliary materials (e.g. lubricants),
and electric power consumption - including material
Comparability and energy flows contributing less than 1 % of mass or
Basically, a comparison or an evaluation of EPD data energy (if available). It can be justified, that all
is only possible if all the data sets to be compared excluded flows contribute less than 5% to the impact
were created according to EN 15804 and the building assessment categories.
context, respectively the product-specific
characteristics of performance, are taken into account. Impacts relating to the production of machines and
facilities required during production are out of the
Background database: GaBi, SP40. scope of this assessment.
Cut-off criteria Period under review
The period under review is 12-months of the calendar
year 2020.
LCA: Scenarios and additional technical information
Characteristic product properties
Information on biogenic Carbon
Information on describing the biogenic Carbon
Content at factory gate
Name Value Unit
Biogenic Carbon Content in
0 kg C
product
Biogenic Carbon Content in
accompanying packaging 0.7 kg C
Cardboard box
The Following Technical information is a basis of the
declared modules and can be used for developing
specific scenarios in the context of a building
assessment if modules are not declared.
Transport to the building site (A4)
Name Value Unit
Litres of fuel 0.57 l/100km
Transport distance 1000 km
Capacity utilisation volume factor
0.53 -
(utilisation by mass)
Installation into the building (A5)
Name Value Unit
Incineration (PVC packaging) 0.76 kg
Incineration (Cardboard packaging) 1.28 kg
Reference service life
Name Value Unit
Life Span according to the
30 a
manufacturer
End of life (C1-C4)
Name Value Unit
Collected separately 73.046 kg
Energy recovery 0 kg
Landfilling (Other core materials) 4.61 kg
Landfilling (Steel) 11.4 kg
Transport Distance (To recycling site) 50 km
Reuse, recovery and/or recycling potentials (D),
relevant scenario information
Name Value Unit
Recycling of steel 64.55 kg
4 Environmental Product Declaration France Metal – Medallion Door
LCA: Results
Results shown below were calculated according to EN 15804 +A2 standard.
In Table 1 "Description of the system boundary", all declared modules shall be indicated with an "X"; all modules
that are not declared shall be indicated with "MND" (As default the modules B3, B4, B5 are marked as MNR –
module not relevant).
Note: The results declared for EP-freshwater are declared in the unit “P eq.” according to the European Platform
on Life Cycle Assessment (http://eplca.jrc.ec.europa.eu/LCDN/developerEF.xhtml). This web link is provided in
EN 15804+A2, clause 6.3.8.2.
DESCRIPTION OF THE SYSTEM BOUNDARY (X = INCLUDED IN LCA; ND = MODULE OR INDICATOR NOT
DECLARED; MNR = MODULE NOT RELEVANT)
BENEFITS AND
CONSTRUCTI LOADS
PRODUCT STAGE ON PROCESS USE STAGE END OF LIFE STAGE BEYOND THE
STAGE SYSTEM
BOUNDARIES
5 Environmental Product Declaration France Metal – Medallion Door
lairetam
waR
ylppus tropsnarT
gnirutcafunaM
eht
morf
tropsnarT
etis
eht
ot
etag
ylbmessA esU
ecnanetniaM
riapeR
tnemecalpeR tnemhsibrufeR
ygrene
lanoitarepO esu
retaw
lanoitarepO esu
noitcurtsnoc-eD
noitilomed tropsnarT
gnissecorp
etsaW
lasopsiD -esueR -yrevoceR -gnilcyceR laitnetop
A1 A2 A3 A4 A5 B1 B2 B3 B4 B5 B6 B7 C1 C2 C3 C4 D
X X X X X ND ND MNR MNR MNR ND ND X X X X X
RESULTS OF THE LCA - ENVIRONMENTAL IMPACT according to EN 15804+A2: 1 Unit Medallion Steel
Door
Core Indicator Unit A1-A3 A4 A5 C1 C2 C3 C4 D
GWP-total [kg CO2-Eq.] 2.56E+2 2.17E+1 4.61E+0 0.00E+0 1.08E+0 0.00E+0 2.24E-1 -1.03E+2
GWP-fossil [kg CO2-Eq.] 2.58E+2 2.08E+1 2.02E+0 0.00E+0 1.03E+0 0.00E+0 2.43E-1 -1.03E+2
GWP-biogenic [kg CO2-Eq.] -1.44E+0 9.19E-1 2.59E+0 0.00E+0 4.56E-2 0.00E+0 0.00E+0 -6.61E-2
GWP-luluc [kg CO2-Eq.] 6.56E-2 1.96E-4 4.31E-4 0.00E+0 9.73E-6 0.00E+0 6.99E-4 1.47E-2
ODP [kg CFC11-Eq.] 1.33E-10 3.17E-16 3.33E-15 0.00E+0 1.57E-17 0.00E+0 9.00E-16 -1.70E-13
AP [mol H+-Eq.] 8.87E-1 2.20E-2 1.09E-3 0.00E+0 1.09E-3 0.00E+0 1.74E-3 -1.91E-1
EP-freshwater [kg PO4-Eq.] 2.06E-4 5.46E-6 5.69E-7 0.00E+0 2.71E-7 0.00E+0 4.17E-7 -2.08E-5
EP-marine [kg N-Eq.] 1.78E-1 4.73E-3 3.77E-4 0.00E+0 2.34E-4 0.00E+0 4.48E-4 -2.84E-2
EP-terrestrial [mol N-Eq.] 1.95E+0 5.42E-2 4.65E-3 0.00E+0 2.68E-3 0.00E+0 4.92E-3 -2.78E-1
POCP [kg NMVOC-Eq.] 6.02E-1 1.68E-2 1.04E-3 0.00E+0 8.32E-4 0.00E+0 1.36E-3 -1.43E-1
ADPE [kg Sb-Eq.] 1.01E-3 1.98E-7 4.83E-8 0.00E+0 9.84E-9 0.00E+0 2.18E-8 -2.22E-4
ADPF [MJ] 2.80E+3 2.91E+2 4.21E+0 0.00E+0 1.44E+1 0.00E+0 3.18E+0 -9.04E+2
[m³ world-Eq
WDP 5.64E+1 3.36E-2 3.77E-1 0.00E+0 1.66E-3 0.00E+0 2.54E-2 -2.02E+1
deprived]
GWP = Global warming potential; ODP = Depletion potential of the stratospheric ozone layer; AP = Acidification potential of land and water; EP =
Caption Eutrophication potential; POCP = Formation potential of tropospheric ozone photochemical oxidants; ADPE = Abiotic depletion potential for non-
fossil resources; ADPF = Abiotic depletion potential for fossil resources; WDP = Water (user) deprivation potential
RESULTS OF THE LCA - INDICATORS TO DESCRIBE RESOURCE USE according to EN 15804+A2: 1 Unit
Medallion Steel Door
Indicator Unit A1-A3 A4 A5 C1 C2 C3 C4 D
PERE [MJ] 1.48E+2 1.53E-1 2.01E+1 0.00E+0 7.57E-3 0.00E+0 4.17E-1 8.10E+1
PERM [MJ] 1.92E+1 0.00E+0 -1.92E+1 0.00E+0 0.00E+0 0.00E+0 0.00E+0 0.00E+0
PERT [MJ] 1.67E+2 1.53E-1 8.58E-1 0.00E+0 7.57E-3 0.00E+0 4.17E-1 8.10E+1
PENRE [MJ] 2.77E+3 2.91E+2 1.79E+1 0.00E+0 1.44E+1 0.00E+0 2.49E+1 -9.04E+2
PENRM [MJ] 3.54E+1 0.00E+0 -1.37E+1 0.00E+0 0.00E+0 0.00E+0 -2.17E+1 0.00E+0
PENRT [MJ] 2.80E+3 2.91E+2 4.21E+0 0.00E+0 1.44E+1 0.00E+0 3.19E+0 -9.04E+2
SM [kg] 5.20E+0 0.00E+0 0.00E+0 0.00E+0 0.00E+0 0.00E+0 0.00E+0 6.91E+1
RSF [MJ] 0.00E+0 0.00E+0 0.00E+0 0.00E+0 0.00E+0 0.00E+0 0.00E+0 0.00E+0
NRSF [MJ] 0.00E+0 0.00E+0 0.00E+0 0.00E+0 0.00E+0 0.00E+0 0.00E+0 0.00E+0
FW [m³] 1.54E+0 1.01E-3 9.30E-3 0.00E+0 5.01E-5 0.00E+0 8.03E-4 -4.54E-1
PERE = Use of renewable primary energy excluding renewable primary energy resources used as raw materials; PERM = Use of
renewable primary energy resources used as raw materials; PERT = Total use of renewable primary energy resources; PENRE = Use of
non-renewable primary energy excluding non-renewable primary energy resources used as raw materials; PENRM = Use of non-
Caption
renewable primary energy resources used as raw materials; PENRT = Total use of non-renewable primary energy resources; SM = Use
of secondary material; RSF = Use of renewable secondary fuels; NRSF = Use of non-renewable secondary fuels; FW = Use of net fresh
water
RESULTS OF THE LCA – WASTE CATEGORIES AND OUTPUT FLOWS according to EN 15804+A2:
1 Unit Medallion Steel Door
Indicator Unit A1-A3 A4 A5 C1 C2 C3 C4 D
HWD [kg] 3.08E-6 1.50E-8 1.73E-8 0.00E+0 7.44E-10 0.00E+0 4.86E-8 2.44E-7
NHWD [kg] 1.50E+1 2.63E-3 1.27E+0 0.00E+0 1.30E-4 0.00E+0 1.60E+1 1.07E+1
RWD [kg] 6.60E-3 3.08E-5 1.46E-4 0.00E+0 1.53E-6 0.00E+0 3.62E-5 3.10E-5
CRU [kg] 0.00E+0 0.00E+0 0.00E+0 0.00E+0 0.00E+0 0.00E+0 0.00E+0 0.00E+0
MFR [kg] 6.38E+0 0.00E+0 0.00E+0 0.00E+0 0.00E+0 5.82E+1 0.00E+0 0.00E+0
MER [kg] 0.00E+0 0.00E+0 2.04E+0 0.00E+0 0.00E+0 0.00E+0 0.00E+0 0.00E+0
EEE [MJ] 0.00E+0 0.00E+0 3.76E+0 0.00E+0 0.00E+0 0.00E+0 0.00E+0 0.00E+0
EET [MJ] 0.00E+0 0.00E+0 6.84E+0 0.00E+0 0.00E+0 0.00E+0 0.00E+0 0.00E+0
HWD = Hazardous waste disposed; NHWD = Non-hazardous waste disposed; RWD = Radioactive waste disposed; CRU = Components
Caption for re-use; MFR = Materials for recycling; MER = Materials for energy recovery; EEE = Exported electrical energy; EET = Exported
thermal energy
RESULTS OF THE LCA – additional impact categories according to EN 15804+A2-optional:
1 Unit Medallion Steel Door
Indicator Unit A1-A3 A4 A5 C1 C2 C3 C4 D
[Disease
PM 1.10E-5 1.28E-7 1.69E-8 0.00E+0 6.35E-9 0.00E+0 2.16E-8 -3.15E-6
Incidence]
[kBq U235-
IRP 2.88E+0 2.53E-3 1.64E-2 0.00E+0 1.25E-4 0.00E+0 3.72E-3 2.67E+0
Eq.]
ETP-fw [CTUe] 5.38E+2 8.75E+1 3.29E+0 0.00E+0 4.34E+0 0.00E+0 1.83E+0 4.72E-1
HTP-c [CTUh] 5.70E-8 1.48E-9 1.34E-10 0.00E+0 7.32E-11 0.00E+0 2.70E-10 3.41E-8
HTP-nc [CTUh] 3.72E-6 4.73E-8 1.32E-8 0.00E+0 2.34E-9 0.00E+0 2.97E-8 -1.39E-6
SQP [-] 5.45E+2 1.33E-1 9.76E-1 0.00E+0 6.62E-3 0.00E+0 6.64E-1 3.39E+1
PM = Potential incidence of disease due to PM emissions; IR = Potential Human exposure efficiency relative to U235; ETP-fw = Potential
Caption comparative Toxic Unit for ecosystems; HTP-c = Potential comparative Toxic Unit for humans (cancerogenic); HTP-nc = Potential
comparative Toxic Unit for humans (not cancerogenic); SQP = Potential soil quality index
Disclaimer 1 – for the indicator “Potential Human exposure efficiency relative to U235”. This impact category
deals mainly with the eventual impact of low dose ionizing radiation on human health of the nuclear fuel cycle. It
does not consider effects due to possible nuclear accidents, occupational exposure nor radioactive waste
disposal in underground facilities. Potential ionizing radiation from the soil, from radon and from some
construction materials is also not measured by this indicator.
Disclaimer 2 – for the indicators “abiotic depletion potential for non-fossil resources”, “abiotic depletion potential
for fossil resources”, “water (user) deprivation potential, deprivation-weighted water consumption”, “potential
comparative toxic unit for ecosystems”, “potential comparative toxic unit for humans – cancerogenic”, “Potential
comparative toxic unit for humans - not cancerogenic”, “potential soil quality index”. The results of this
environmental impact indicator shall be used with care as the uncertainties on these results are high or as there is
limited experience with the indicator.
References
Standards BS 476 Part 22:1987, Fire tests on building materials
and structures,
ANSI/UL10B Part 22: Methods for determination of the fire
ANSI/UL10B: 2020, UL Standard for Safety Fire Tests resistance of non-loadbearing elements of
of Door Assemblies: Underwriters Laboratories Inc. construction.
(UL).
DIN EN 1634-1
ANSI/UL10C DIN EN 1634-1: 2018, Fire resistance and smoke
ANSI/UL10C:2016, UL Standard for Safety Positive control tests for door and shutter assemblies, openable
Pressure Fire Tests of Door Assemblies: Underwriters windows and elements of building hardware - Part 1
Laboratories Inc. (UL). including Amendment A1:2018: Fire resistance test for
door and shutter assemblies and openable windows
ASTM E90
ASTM E90-09:2016, EN 15804 +A2
Standard Test Method for Laboratory Measurement of EN 15804 +A2: 2019, Sustainability of construction
Airborne Sound Transmission Loss of Building works — Environmental Product Declarations — Core
Partitions and Elements, The American Society for rules for the product category of construction products.
Testing and Materials.
ISO 15686
ASTM E238 ISO 15686:2011-05, Buildings and constructed assets
ASTM E238-17a: 2017, Standard Test Method for Pin- - Service life planning
Type Bearing Test of Metallic, The American Society
for Testing and Materials. ISO 14025
DIN EN ISO 14025:2011-10, Environmental labels and
BS 476 Part 22 declarations — Type III environmental declarations —
Principles and procedures.
6 Environmental Product Declaration France Metal – Medallion Door
IBU
EN 16034 Institut Bauen und Umwelt e.V.: General Programme
EN 16034:2014,Pedestrian doorsets, industrial, Instructions for the Preparation of EPDs at the Institut
commercial, garage doors and openable windows. Bauen und Umwelt e.V. Version 1., Berlin: Institut
Product standard, performance characteristics. Fire Bauen und Umwelt e.V., 2016. www.ibu-epd.com
resisting and/or smoke control characteristics.
PCR guideline texts for building-related
Further References products and services (PCR)
Candidate list PCR - Part A: Calculation Rules for the Life Cycle As-
List of those eligible for approval substances of very sessment and Requirements on the Project Report,
high concern to the European Chemicals Agency, as of version 1.8, Institut Bauen und Umwelt e.V., www.bau-
December 22, 2021. umwelt.com, 2019
CPR PCR – Part B: Requirements of the EPD for windows
Regulation (EU) No. 305/2011 Construction Product and doors , version 1.7, Institut Bauen und Umwelt
Regulation (CPR). e.V., www.bau-umwelt.com, 2019
(EU) Ordinance on Biocide Products No. 528/2012 REACH Regulation
Regulation (EU) No 528/2012 of the European (EC) No. 1907/2006 of the European Parliament and
Parliament and of the Council of 22 May 2012 Council of December 18, 2006 for Registration,
concerning the making available on the market and evaluation, admission and Restriction of chemical
use of biocidal products Text with EEA relevance. substances. List of those eligible for approval
substances of very high concern to the European
GaBi ts v10.6.0.110 Chemicals Agency, as of June 25, 2020.
Software & Documentation (CUP 2020.2), 2020
Sphera solutions GmBH,
Documentation of GaBi data sets
http://www.gabi-software.com/international/databases/
7 Environmental Product Declaration France Metal – Medallion Door
Publisher
Institut Bauen und Umwelt e.V. Tel +49 (0)30 3087748- 0
Panoramastr. 1 Fax +49 (0)30 3087748- 29
10178 Berlin Mail info@ibu-epd.com
Germany Web www.ibu-epd.com
Programme holder
Institut Bauen und Umwelt e.V. Tel +49 (0)30 - 3087748- 0
Panoramastr 1 Fax +49 (0)30 – 3087748 - 29
10178 Berlin Mail info@ibu-epd.com
Germany Web www.ibu-epd.com
Author of the Life Cycle
Assessment Tel +49 711 341817-0
Sphera Solutions GmbH Fax +49 711 341817-25
Hauptstraße 111- 113 Mail info@sphera.com
70771 Leinfelden-Echterdingen Web www.sphera.com
Germany
Owner of the Declaration
French Company for Metallic Tel +20222564293
Industries Fax +20222564294
Shafik Ghorbal St., Roxy 9A Mail info@francemetal.net
11341 Cairo Web www.francemetal.net
Egypt
