ENVIRONMENTAL PRODUCT DECLARATION
as per ISO 14025 and EN 15804+A2
Owner of the Declaration dormakaba International Holding GmbH
Publisher Institut Bauen und Umwelt e.V. (IBU)
Programme holder Institut Bauen und Umwelt e.V. (IBU)
Declaration number EPD-DOR-20210315-CBA8-EN
Issue date 25.02.2022
Valid to 24.02.2027
ARGUS AIR sensor barriers
dormakaba
www.ibu-epd.com | https://epd-online.com
General Information
dormakaba ARGUS AIR sensor barriers
Programme holder Owner of the declaration
IBU – Institut Bauen und Umwelt e.V. dormakaba International Holding GmbH
Hegelplatz 1 DORMA Platz 1
10117 Berlin 58256 Ennepetal
Germany Germany
Declaration number Declared product / declared unit
EPD­DOR­20210315­CBA8­EN 1 piece of the product: one (1) dormakaba ARGUS Air Lounge sensor
barrier, consisting of the following items:
­ housing
­ tempered safety glasses (6mm)
­ cover plates
­ glass door leaves (10mm)
­ drive unit
­ sensor technology
­ LED status display
­ product packaging
This declaration is based on the product category rules: Scope:
Electronic and physical Access Control Systems, 01.08.2021 This EPD is a specific product decalaration for the ARGUS AIR Lounge
(PCR checked and approved by the SVR) sensor barriers. It is also representative for the ARGUS AIR Security and
ARGUS AIR Boarding sensor barriers. The underlying life cycle
assessment is based on the entire life cycle of this specific ARGUS Air
Issue date Lounge sensor barrier. The products are manufactured at the dormakaba
production facility in Bühl (Germany). Green electricity is being used at this
25.02.2022
production site.
Data represents the year 2021.
The owner of the declaration shall be liable for the underlying information
Valid to
and evidence; the IBU shall not be liable with respect to manufacturer
24.02.2027 information, life cycle assessment data and evidences.
The EPD was created according to the specifications of EN 15804+A2. In
the following, the standard will be simplified as EN 15804.
Verification
The standard EN 15804 serves as the core PCR
Independent verification of the declaration and data according to ISO
14025:2011
internally X externally
Dipl.­Ing. Hans Peters
(Chairman of Institut Bauen und Umwelt e.V.)
Florian Pronold Dr.­Ing. Wolfram Trinius,
(Managing Director Institut Bauen und Umwelt e.V.) (Independent verifier)
1 Environmental Product Declaration ­ dormakaba ­ ARGUS AIR sensor barriers
Product
Product description/Product definition
Argus Air
eGates Argus Air for fast, safe passenger flow at airports. Argus
Air supports passengers and staff during the entire process,
from entering the airport to the aircraft. The sensor barriers with
their narrow and short design ensure a fast flow of passengers
at the airports and smooth, comfortable processes.
The Argus Air series includes the gates for boarding pass
control Argus Air Security, lounge access Argus Air Lounge and
for self­boarding Argus Air Boarding.
Argus Air Boarding
The Argus Air Boarding ensures effective, comfortable boarding
for passengers. Control system and power supply integrated into the unit.
Dimensions of Argus Air Lounge
Argus Air Security
Name Value Unit
Argus Air Security with its biometric face recognition, combines
a high level of security with a smooth and effective passenger Height Dimension 990 mm
flow. Length Dimension 1650 mm
Passege width Dimension 540 mm
Argus Air Lounge
Overall width Dimension 1051 mm
The Argus Air Lounge with its intuitive, contactless operation
Guiding element width Dimension 180 mm
guarantees easy access to lounges, even with luggage,
children or wheelchairs. For the placing on the market in the The Argus Air Lounge includes the following components:
European Union/European Free Trade Associaton (EU/EFTA) ­ two (2) housing
(with the exception of Switzerland) the following legal provisions ­ two (2) tempered safety glasses (6mm)
apply: ­ two (2) cover plates
­ two (2) glass door leaves (10mm)
• Machinery Directive 2006/42/EC
­ one (1) drive unit
• 2014/30/EU Electromagnetic Compatibility Directive
­ sensor technology
• 2011/65/EU ROHS2 Directive
­ LED status display
• DIN EN ISO 12100:2011-03 Safety of machinery
­ packaging material
• DIN EN 16005: 2013-01 and Amendment 2015-10
The total weight of all components is 256,05 kg including
Power operated pedestrian doorsets
packaging 294,95 kg.
• DIN EN ISO 13849- 1:2016-06 Safety of machinery
• DIN EN ISO 13849- 2:2013-02 Safety of machinery
Product not harmonised in accordance with the
• DIN EN 60335-2-103: 2016-05 Household and similar
CPR but in accordance with other provisions for harmonisation
electrical appliances
of the EU:
• DIN EN 61000-3-2:2015-03 Electromagnetic
compatibility (EMC) • Machinery Directive 2006/42/EC
• DIN EN 61000-6-2: 2005 and Amendment:2011 • 2014/30/EU Electromagnetic Compatibility Directive
Electromagnetic Compatibility (EMC) • 2011/65/EU ROHS2 Directive
• DIN EN 61000-6-3:2007 and A1:2011 Electromagnetic • DIN EN ISO 12100:2011-03 Safety of machinery
Compatibility (EMC) • DIN EN 16005: 2013-01 and Amendment 2015-10
The CE­marking takes into account the proof of conformity with Power operated pedestrian doorsets
the respective harmonized standards based on the legal • DIN EN ISO 13849- 1:2016-06 Safety of machinery
provisions above. • DIN EN ISO 13849- 2:2013-02 Safety of machinery
• DIN EN 60335-2-103: 2016-05 Household and similar
For the application and use the respective national provisions electrical appliances
apply. • DIN EN 61000-3-2:2015-03 Electromagnetic
compatibility (EMC)
Application
• DIN EN 61000-6-2: 2005 and Amendment:2011
Argus Air sensor gates can be used for convenient entry into: Electromagnetic Compatibility (EMC)
• Airports • DIN EN 61000-6-3:2007 and A1:2011 Electromagnetic
The different sensor gates ensure a reliable boarding, control Compatibility (EMC)
when entering the business lounge or access control at the
Base materials/Ancillary materials
passenger entrance to the security area.
For the main Argus Air Lounge product components the
Technical Data composition is the following. The same product composition
The sensor barriers Argus Air Security, Boarding and Lounge applies for Argus Air Boarding and Argus Air Security:
have the following technical properties:
The composition of the Argus Air Lounge is listed in the
following table:
2 Environmental Product Declaration ­ dormakaba ­ ARGUS AIR sensor barriers
listed in the Candidate List of REACH Regulation
1907/2006/EC (date: 19.01.2021)
exceeding 0.1 percentage by mass: yes
• Lead (Pb): 7439­921­1 (CAS­No.) is included in some of
the alloys used. The concentration of lead in each
individual alloy does not exceed 0,35 % (by mass).
The Candidate List can be found on the /ECHA/ website
address: https://echa.europa.eu/de/home.
Reference service life
The life cycle of an ARGUS Air is about 10 years, depending on
the application and frequency of use. The ARGUS Air is tested
according to EN 16005.
The product contains partial articles which contain substances
LCA: Calculation rules
Declared Unit Use stage - Module B6
The declared unit is 1 piece of product: 256.05 kg The use stage related to the operation of the building includes:
Name Value Unit — B6, operational energy use
Declared unit 1 pce.
End-of-life stage– Modules C1-C4 and D
Mass (total system excluding packaging) 256 kg
The end­of­life stage includes:
— C1, de­construction, demolition;
System boundary
— C2, transport to waste processing;
Type of EPD:
— C3, waste processing for reuse, recovery and/or recycling;
cradle to gate with options, modules C1–C4, and module D
— C4, disposal; including provision and all transport, provision
(A1–A3 + C + D and additional modules: A4 + A5 + B6)
of all materials, products and related energy and water use.
— D, (Benefits and loads beyond the system boundary)
Production - Module A1-A3
includes: recycling potentials, expressed as net impacts and
The product stage includes:
benefits.
— A1, raw material extraction, processing and mechanical
treatments, processing of secondary material input (e.g. Geographic Representativeness
recycling processes), Land or region, in which the declared product system is
— A2, transport to the manufacturer, manufactured, used or handled at the end of the product´s
— A3, manufacturing and assembly including provision of all lifespan: Germany
materials, products and energy, as well as waste processing up
to the end­of waste state.
Comparability
Construction stage - Modules A4-A5 Basically, a comparison or an evaluation of EPD data is only
The construction process stage includes: possible if all the data sets to be compared were created
— A4, transport to the building site; according to EN 15804 and the building context, respectively
— A5, installation into the building; including provision of all the product­specific characteristics of performance, are taken
materials, products and energy, as well as waste processing up into account.
to the end of waste state or disposal of final residues during the
construction process stage.
LCA: Scenarios and additional technical information
Installation into the building (A5)
Characteristic product properties of biogenic carbon
Name Value Unit
Information on describing the biogenic Carbon Content at
Waste packaging (paper and plastic) 38.9 kg
factory gate
Name ValueUnit Reference service life
Biogenic carbon content in product 1.69 kg Name Value Unit
C
Life Span according to the manufacturer 10 a
Biogenic carbon content in accompanying kg
14.45
packaging C Operational energy use (B6)
The use stage is declared for 10 years
The following technical scenario information is required Name Value Unit
for the declared modules Days per year in use 365 days
Transport to the building site (A4) On mode per day 2 hours
Name Value Unit Idle mode per day 22 hours
Litres of fuel (per 1 kg) 0.00276 l/100km On mode power 78 W
Capacity utilisation (including empty runs) 55 % Idle mode power 64 W
Transport distance via medium truck 100 km Electricity consumption (per 1 year) 570.86 kWh
3 Environmental Product Declaration ­ dormakaba ­ ARGUS AIR sensor barriers
electromechanics. The plastic components are assumed to be
End of life (C1-C4)
incinerated with energy recovery. Minor proportions of residues
Name Value Unit
arising from the recycling process are landfilled (1%). Region
Recycling 163.89 kg for the End of Life is: Global.
Energy recovery 4.46 kg
Landfilling 87.7 kg Reuse, recovery and/or recycling potentials (D), relevant
scenario information
Transport to waste management 50 km
Collection rate is 100%.
The product is disassembled in a recycling process. Material
recycling is then assumed for the metals, electronic and
4 Environmental Product Declaration ­ dormakaba ­ ARGUS AIR sensor barriers
LCA: Results
DESCRIPTION OF THE SYSTEM BOUNDARY (X = INCLUDED IN LCA; MND = MODULE OR INDICATOR NOT DECLARED; MNR
= MODULE NOT RELEVANT)
Benefits and
Construction loads beyond
Product stage Use stage End of life stage
process stage the system
boundaries
la ire ta m w a Ry lp p u s tro p s n a rT g n iru tc a fu n a M e h t m o rf tro p s n a rTe tis e h t o t e ta g y lb m e s s A e s U e c n a n e tn ia M ria p e R tn e m e c a lp e R tn e m h s ib ru fe R y g re n e la n o ita re p Oe s u re ta w la n o ita re p Oe s u n o itc u rts n o c ­e Dn o itilo m e d tro p s n a rT g n is s e c o rp e ts a W la s o p s iD ­e s u e R­y re v o c e R­g n ilc y c e Rla itn e to p
A1 A2 A3 A4 A5 B1 B2 B3 B4 B5 B6 B7 C1 C2 C3 C4 D
X X X X X MND MND MNR MNR MNR X MND X X X X X
RESULTS OF THE LCA - ENVIRONMENTAL IMPACT according to EN 15804+A2: 1 piece Argus Air sensor barriers
Parameter Unit A1-A3 A4 A5 B6 C1 C2 C3 C4 D
GWP­total kg CO 2 eq 1.54E+03 2.58E+00 6.3E+01 2.31E+03 0 1.12E+00 1.97E+01 1.34E+00 ­9.18E+02
GWP­fossil kg CO 2 eq 1.59E+03 2.47E+00 8.53E+00 2.3E+03 0 1.07E+00 1.15E+01 1.33E+00 ­9.15E+02
GWP­biogenic kg CO 2 eq ­5.76E+01 1.14E­01 5.45E+01 7.66E+00 0 4.95E­02 8.24E+00 4.55E­03 ­2.47E+00
GWP­luluc kg CO 2 eq 8.83E­01 5.87E­05 1.2E­03 3.33E+00 0 2.55E­05 7.21E­04 3.83E­03 ­2.64E­01
ODP kg CFC11 eq 7.25E­09 2.6E­16 1.25E­14 5.05E­11 0 1.13E­16 6.73E­15 4.93E­15 ­6.69E­09
AP mol H+ eq 8.19E+00 2.47E­03 1.29E­02 5.07E+00 0 1.07E­03 3.22E­03 9.54E­03 ­3.64E+00
EP­freshwater kg P eq 1.85E­03 5.28E­07 2.21E­06 6.14E­03 0 2.29E­07 1.06E­06 2.29E­06 ­5.29E­04
EP­marine kg N eq 1.22E+00 7.85E­04 4.01E­03 1.13E+00 0 3.41E­04 8.45E­04 2.46E­03 ­4.86E­01
EP­terrestrial mol N eq 1.34E+01 8.73E­03 5.55E­02 1.18E+01 0 3.79E­03 1.48E­02 2.7E­02 ­5.28E+00
kg NMVOC
POCP 3.5E+00 2.22E­03 1.08E­02 3.09E+00 0 9.65E­04 2.32E­03 7.44E­03 ­1.52E+00
eq
ADPE kg Sb eq 3.83E­02 7.39E­08 1.9E­07 6.65E­04 0 3.21E­08 9.46E­08 1.19E­07 ­2.07E­02
ADPF MJ 2.1E+04 3.5E+01 1.87E+01 4.04E+04 0 1.52E+01 7.05E+00 1.75E+01 ­1.31E+04
m3 world eq
WDP 2.53E+02 4.83E­03 7.15E+00 5.01E+02 0 2.1E­03 2.02E+00 1.39E­01 ­6.59E+01
deprived
GWP = Global warming potential; ODP = Depletion potential of the stratospheric ozone layer; AP = Acidification potential of land and water; EP =
Eutrophication potential; POCP = Formation potential of tropospheric ozone photochemical oxidants; ADPE = Abiotic depletion potential for non­fossil
resources; ADPF = Abiotic depletion potential for fossil resources; WDP = Water (user) deprivation potential)
RESULTS OF THE LCA - INDICATORS TO DESCRIBE RESOURCE USE according to EN 15804+A2: 1 piece Argus Air sensor
barriers
Parameter Unit A1-A3 A4 A5 B6 C1 C2 C3 C4 D
PERE MJ 8.17E+03 1.1E­01 4.58E+02 1.79E+04 0 4.79E­02 5.69E+01 2.29E+00 ­5.97E+03
PERM MJ 5.09E+02 0 ­4.54E+02 0 0 0 ­5.52E+01 0 0
PERT MJ 8.68E+03 1.1E­01 3.72E+00 1.79E+04 0 4.79E­02 1.7E+00 2.29E+00 ­5.97E+03
PENRE MJ 2.07E+04 3.5E+01 1.43E+02 4.04E+04 0 1.52E+01 1.65E+02 1.75E+01 ­1.31E+04
PENRM MJ 2.83E+02 0 ­1.25E+02 0 0 0 ­1.58E+02 0 0
PENRT MJ 2.1E+04 3.5E+01 1.87E+01 4.04E+04 0 1.52E+01 7.05E+00 1.75E+01 ­1.31E+04
SM kg 1.32E+01 0 0 0 0 0 0 0 0
RSF MJ 0 0 0 0 0 0 0 0 0
NRSF MJ 0 0 0 0 0 0 0 0 0
FW m3 1.93E+01 1.98E­04 1.69E­01 2.07E+01 0 8.6E­05 4.8E­02 4.4E­03 ­1.1E+01
PERE = Use of renewable primary energy excluding renewable primary energy resources used as raw materials; PERM = Use of renewable primary
energy resources used as raw materials; PERT = Total use of renewable primary energy resources; PENRE = Use of non­renewable primary energy
excluding non­renewable primary energy resources used as raw materials; PENRM = Use of non­renewable primary energy resources used as raw
materials; PENRT = Total use of non­renewable primary energy resources; SM = Use of secondary material; RSF = Use of renewable secondary fuels;
NRSF = Use of non­renewable secondary fuels; FW = Use of net fresh water
RESULTS OF THE LCA – WASTE CATEGORIES AND OUTPUT FLOWS according to EN 15804+A2:
1 piece Argus Air sensor barriers
Parameter Unit A1-A3 A4 A5 B6 C1 C2 C3 C4 D
HWD kg 7.47E­05 3.39E­09 3.32E­08 1.67E­05 0 1.48E­09 2.13E­08 2.66E­07 ­1.19E­05
NHWD kg 3.72E+02 3.58E­03 2.09E+00 2.87E+01 0 1.56E­03 1.24E+00 8.78E+01 ­2.29E+02
RWD kg 1.14E+00 3.76E­05 9.6E­04 6.13E+00 0 1.63E­05 2.98E­04 1.99E­04 ­1.39E+00
CRU kg 0 0 0 0 0 0 0 0 0
MFR kg 0 0 0 0 0 0 1.6E+02 0 0
MER kg 0 0 0 0 0 0 0 0 0
EEE MJ 0 0 9.35E+01 0 0 0 0 0 0
EET MJ 0 0 1.76E+02 0 0 0 0 0 0
5 Environmental Product Declaration ­ dormakaba ­ ARGUS AIR sensor barriers
HWD = Hazardous waste disposed; NHWD = Non­hazardous waste disposed; RWD = Radioactive waste disposed; CRU = Components for re­use;
MFR = Materials for recycling; MER = Materials for energy recovery; EEE = Exported electrical energy; EET = Exported thermal energy
RESULTS OF THE LCA – additional impact categories according to EN 15804+A2-optional:
1 piece Argus Air sensor barriers
Parameter Unit A1-A3 A4 A5 B6 C1 C2 C3 C4 D
Disease
PM 8.64E­05 1.3E­08 8.83E­08 4.26E­05 0 5.64E­09 3.18E­08 1.18E­07 ­5.82E­05
incidence
IR kBq U235 eq 2.19E+02 5.37E­03 1.41E­01 1.01E+03 0 2.33E­03 3.38E­02 2.04E­02 ­2.79E+02
ETP­fw CTUe 9.76E+03 2.48E+01 8.54E+00 1.73E+04 0 1.08E+01 2.76E+00 9.97E+00 ­5.03E+03
HTP­c CTUh 2.13E­05 4.66E­10 5.96E­10 4.77E­07 0 2.03E­10 2.23E­10 1.48E­09 ­2.71E­07
HTP­nc CTUh 2.23E­05 1.99E­08 3.86E­08 1.76E­05 0 8.67E­09 1.91E­08 1.63E­07 1.94E­06
SQP SQP 8.97E+03 8.99E­02 5.19E+00 1.29E+04 0 3.91E­02 2.07E+00 3.64E+00 ­5.12E+02
PM = Potential incidence of disease due to PM emissions; IR = Potential Human exposure efficiency relative to U235; ETP­fw = Potential comparative
Toxic Unit for ecosystems; HTP­c = Potential comparative Toxic Unit for humans (cancerogenic); HTP­nc = Potential comparative Toxic Unit for humans
(not cancerogenic); SQP = Potential soil quality index
Disclaimer 1 – for the indicator 'Potential Human exposure efficiency relative to U235'.
This impact category deals mainly with the eventual impact of low dose ionizing radiation on human health of the nuclear fuel cycle. It
does not consider effects due to possible nuclear accidents, occupational exposure nor radioactive waste disposal in underground
facilities. Potential ionizing radiation from the soil, from radon and from someconstruction materials is also not measured by this
indicator.
Disclaimer 2 – for the indicators 'abiotic depletion potential for non­fossil resources', 'abiotic depletion potential for fossil resources',
'water (user) deprivation potential, deprivation­weighted water consumption', 'potential comparative toxic unit for ecosystems', 'potential
comparative toxic unit for humans – cancerogenic', 'Potential comparative toxic unit for humans ­ not cancerogenic', 'potential soil
quality index'.
The results of this environmental impact indicator shall be used with care as the uncertainties on these results are high or as there is
limited experience with the indicator.
References
Standards hazardous substances in electrical and
electronic equipment
EN 15804
EN 15804:2012+A1 2013, Sustainability of construction works DIN EN ISO 12100
— Environmental Product Declarations — Core rules for the DIN EN ISO 12100:2011­03 Safety of machinery
product category of construction products.
DIN EN ISO 13849- 1
EN 15804 DIN EN ISO 13849­ 1:2016­06 Safety of machinery
EN 15804:2012+A2:2019+AC:2021, Sustainability of
construction works — Environmental Product Declarations — DIN EN ISO 13849- 2
Core rules for the product category of construction products. DIN EN ISO 13849­ 2:2013­02 Safety of machinery
ISO 14025 ISO 14025
EN ISO 14025:2011, Environmental labels and declarations — DIN EN ISO 14025:2011­10, Environmental labels and
Type III environmental declarations — Principles and declarations — Type III environmental declarations —
procedures. Principles and procedures.
Further References EN 15804
EN 15804:2019+A2, Sustainability of construction works —
IBU 2021 Environmental Product
Institut Bauen und Umwelt e.V.: General Instructions for the Declarations — Core rules for the product category of
EPD programme of Institut Bauen und Umwelt e.V., Version construction products.
2.0, Berlin: Institut Bauen und Umwelt e.V., 2021
www.ibu­epd.com DIN EN 16005
DIN EN 16005: 2013­01 and Amendment 2015­10 Power
Machinery Directive operated pedestrian doorsets
DIRECTIVE 2006/42/EC OF THE EUROPEAN PARLIAMENT
AND OF THE COUNCILof 17 May 2006on machinery, and DIN EN 60335-2
amending Directive 95/16/EC DIN EN 60335­2­103: 2016­05 Household and similar electrical
appliances
Electromagnetic Compatibility Directive
DIRECTIVE 2014/30/EU OF THE EUROPEAN PARLIAMENT DIN EN 61000-3-2
AND OF THE COUNCILof 26 February 2014on the DIN EN 61000­3­2:2015­03 Electromagnetic compatibility
harmonisation of the laws of the Member States relating to (EMC)
electromagnetic compatibility
DIN EN 61000-6-2
ROHS2 Directive DIN EN 61000­6­2: 2005 and Amendment:2011
Directive 2011/65/EU of the European Parliament and of the Electromagnetic Compatibility (EMC)
Council of 8 June 2011 on the restriction of the use of certain
6 Environmental Product Declaration ­ dormakaba ­ ARGUS AIR sensor barriers
DIN EN 61000-6-3 University of Stuttgart Leinfelden­Echterdingen
DIN EN 61000­6­3:2007 and A1:2011 Electromagnetic
Compatibility (EMC) GaBi ts documentation
GaBi life cycle inventory data documentation
REACH (https://www.gabisoftware.com/support/gabi/gabidatabase[1]2020
Regulation (EC) No 1907/2006 of the European Parliament and lci­documentation/).
of the Council on the Registration, Evaluation, Authorisation
and Restriction of Chemicals (REACH) LCA-tool dormakaba
LCA tool, version 1.0. ESC (Entrance System Control)
ISO 9001 Developed by Sphera Solutions GmbH.
ISO 9001:2015­09 Quality management systems ­
Requirements PCR Part A
PCR – Part A: Calculation Rules for the Life Cycle Assessment
European Waste Catalogue (EWC) and Requirements on the Project Re­port according to EN
COMMISSION DECISION of 18 December 2014 amending 15804+A2:2019, Version 1.0, Institut Bauen und Umwelt e.V.,
Decision 2000/532/EC on the list of waste pursuant to Directive www.ibu­epd.com, 2020.
2008/98/EC of the European Parliament and of the Council
PCR Part B
Further References PCR – Part B:
Requirements on the EPD for electronic and physical Access
GaBi ts software Control Systems, version, 08/2021, Institut Bauen und Umwelt
Sphera Solutions GmbH Gabi Software System and Database e.V., www.ibu­epd.com
for Life Cycle Engineering 1992­2020 Version 10.0.0.71
7 Environmental Product Declaration ­ dormakaba ­ ARGUS AIR sensor barriers
Publisher
Institut Bauen und Umwelt e.V. +49 (0)30 3087748­ 0
Hegelplatz 1 info@ibu­epd.com
10117 Berlin www.ibu­epd.com
Germany
Programme holder
Institut Bauen und Umwelt e.V. +49 (0)30 3087748­ 0
Hegelplatz 1 info@ibu­epd.com
10117 Berlin www.ibu­epd.com
Germany
Author of the Life Cycle Assessment
Sphera Solutions GmbH +49 711 341817­0
Hauptstraße 111­ 113 info@sphera.com
70771 Leinfelden­Echterdingen www.sphera.com
Germany
Owner of the Declaration
dormakaba International Holding GmbH +49 2333 793­0
DORMA Platz 1 info.de@dormakaba.com
58256 Ennepetal www.dormakaba.com
Germany
8 Environmental Product Declaration ­ dormakaba ­ ARGUS AIR sensor barriers
