ENVIRONMENTAL PRODUCT DECLARATION
as per ISO 14025 and EN 15804+A2
Owner of the Declaration Hansgrohe Group
Programme holder Institut Bauen und Umwelt e.V. (IBU)
Publisher Institut Bauen und Umwelt e.V. (IBU)
Declaration number EPD-HAN-20230025-ICC1-EN
Issue date 24.02.2023
Valid to 23.02.2028
Basic sets
Hansgrohe Group
www.ibu-epd.com | https://epd-online.com
Umwelt Produktdeklaration Name des Herstellers – Name des Produkts
1. General Information
Hansgrohe Group Basic Sets
Programme holder Owner of the declaration
IBU – Institut Bauen und Umwelt e.V. Hansgrohe Group
Hegelplatz 1 Auestraße 5 - 9
10117 Berlin 77761 Schiltach
Germany Germany
Declaration number Declared product / declared unit
EPD-HAN-20230025-ICC1-EN One (1) piece of an average basic set incl. packaging
This declaration is based on the product Scope:
category rules: This average EPD was determined on the basis of a
Fittings and showers, 07.2014 weighted average of production volume from 2020 and
(PCR checked and approved by the SVR) relates to the plants in Wasselonne, France, Offenburg
and Schiltach, Germany and Alpharetta, USA. This
average EPD is valid for the whole product group basic
Issue date
sets. The EPD was formed from >98% of the products
24.02.2023
involved in the sales quantity.
Valid to
The owner of the declaration shall be liable for the
23.02.2028
underlying information and evidence; the IBU shall not
be liable with respect to manufacturer information, life
cycle assessment data and evidences.
The EPD was created according to the specifications
of EN 15804+A2. In the following, the standard will be
simplified as EN 15804.
Verification
The standard EN 15804 serves as the core PCR
Independent verification of the declaration and data
according to ISO 14025:2011
Dipl. Ing. Hans Peters internally x externally
(chairman of Institut Bauen und Umwelt e.V.)
Dr. Alexander Röder Dr Naeem Adibi
(Managing Director Institut Bauen und Umwelt e.V.)) (Independent verifier)
2. Product
2.1 Product description/Product definition  ISO 3822: Acoustics – Laboratory tests on
Basic Sets essentially comprise of brass materials and noise emission from appliances and
several assembly parts of various materials.
equipment used in water supply installations
For the use and application of the product the
respective national provisions at the place of use 2.2 Application
apply, in Germany for example the building codes of Basic Sets are plumbing fixtures that direct water to
the federal states and the corresponding national the end-user products. They are located concealed in
specifications. the wall and need further products (end-user products)
to work. The products are used in bathrooms and rest
The products comply with the applicable standards and rooms. Examples for end-user products are
regulations listed below. thermostats, overhead showers or shower faucets.
Following standards depending on the operating 2.3 Technical Data
mechanism may apply to taps and roughs to prove
product safety:
 EN 816:2017: Sanitary tapware – Automatic Constructional data
Name Value Unit
shut-off valves PN 10
Maximum load temperature permanent
 EN 817:2008: Sanitary tapware – Mechanical 65 °C
operation
mixing valves (PN 10)
Maximum load temperature temporary
90 °C
 EN 200:2008: Sanitary tapware – Single taps operation
and combination taps for water supply Flow rate (indications for pressure Dependi
m3/h
systems of type 1 and type 2 range of 1-3 bar) ng on
2 Environmental Product Declaration Hansgrohe Group – Basic Sets
the No. 2: The body is cast from brass using the sand
product core.
0,09 to No. 3: After casting, the brass body is grinded.
1,2 No. 4: The plastic parts of the body are injected.
Sound emissions < 30 dB No. 5: The product parts are assembled.
No. 6: The preassembled product is packed together
with the remaining components (like enclosed pack).
Performance data of the product with respect to its
characteristics in accordance with the relevant Any production waste generated is disposed
technical provision (no CE-marking). accordingly. In individual cases, the production may
differ slightly from the procedure (for example, if the
2.4 Delivery status brass body is purchased and not manufactured in-
The basic sets are delivered singularly packaged. The house).
packaging is customized to the size of the product and
supplies. Customers can order single products or 2.7 Environment and health during
multiple products with outer packaging. manufacturing
Hansgrohe SE tries to keep the impact on people and
2.5 Base materials/Ancillary materials the environment as low as possible when
manufacturing its products.
The material composition (incl. packaging) of an Hazards at workplaces are regularly assessed and
average basic set is as follows: reduced to a minimum.
For example, in basic production, sawing or grinding
Name Value Unit work is mainly carried out by robots, and in
Brass 59.9 % electroplating, chemicals are dosed automatically via
Cardboard, Paper 17.5 % appropriate pump stations.
Acrylonitrile-butadiene-styrene 10.8 % Emissions that are hazardous to health are extracted
Other plastics 7.0 % directly at the source and cleaned by filter systems.
Workplace and emission limits are regularly monitored
Polyamide 2.2 %
and are far below the prescribed limits.
Stainless steel 1.3 %
To reduce environmental impact, water and production
Other Materials 0.5 %
waste are recycled wherever possible.
Zinc 0.5 %
In addition, all production sites are certified according
to the DIN EN
The parts which are made of brass contain between
ISO standards 14001 (environment), 50001 (energy), 4
0.2 and 1.4% lead.
5001 (occupational health and safety)
This product contains substances listed in the
and 9001 (quality). Continuous improvement of
candidate list (date: 17.12.2021) exceeding 0.1
environmental and occupational safety performance is
percentage by mass: Lead (CAS number 7439-92-1)
thus guaranteed.
as a component of the brass alloy has been on the
candidate list of the Reach Regulation (Regulation
2.8 Product processing/Installation
(EC) No. 1907/2006) since 27.06.2018.
Connect the connection pipes with the basic set (if
necessary, saw the pipes - usually by hand) (tools:
This product/article/at least one partial article contains
vise and wrench).
other CMR substances in categories 1A or 1B which
Fix the basic set on or in the wall and align it (tools:
are not on the candidate list, exceeding 0.1 percentage
vise and wrench).
by mass: no.
Drill a hole for the basic set in cover material (tools:
drilling machine, circular drill bit).
Biocide products were added to this construction
Seal the wall (tool: wrench).
product or it has been treated with biocide products
Apply a sealing sleeve to the supporting wall.
(this then concerns a treated product as defined by the
Drill a hole for the basic set in wall the covering wall
(EU) Ordinance on Biocide Products No.
(tools: drill, circular drill bit) and cover the wall. Seal the
528/2012): no.
basic set (tool: silicone joint).
2.6 Manufacture
2.9 Packaging
For product protection the basic sets are individually
packed in a cardboard box, which consists of
approximately 80% recycled material. The cardboard is
always printed with lead-free ink and in some cases
additionally coated with clear topcoat. The inlay of the
packaging consists of folded cardboard, fiber form or
plastic bags, depending on the product.
The packaging can be fully recycled.
All packaged products fit on a reusable euro pallet.
2.10 Condition of use
There are no unhealthy contaminants in the water
caused by the basic sets.
No. 1: The sand core for the base body is made.
3 Environmental Product Declaration Hansgrohe Group – Basic Sets
2.11 Environment and health during use If a room in which the products offered by Hansgrohe
Our products do not emission any contaminants or are installed is flooded with water, the products are not
substances that are harmful to the environment or affected in their function.
health during the use phase. There will be no environmental impact.
2.12 Reference service life Mechanical destruction
The quality and durability of our basic sets is designed If the surface of the coating is destroyed by a
for a product life of about 20 years and beyond. Which mechanical stress, there is a possibility of corrosion.
on average is approximately the duration of use by the In the event of mechanical damage, the products may
consumers. need to be replaced due to possible sharp cut edges.
With few exceptions, all products have a five-year 2.14 Re-use phase
warranty. Furthermore, an after-sale service warranty The basic sets are not taken back by the manufacturer
of 15 years is provided. for the purpose of reuse.
2.13 Extraordinary effects
2.15 Disposal
Fire The waste code of the product is AVV 20 03 01.
The products are not classified as building materials Disassembly of the products consists of the same
(building products) and are not subject to DIN 4102 steps as assembly, in reverse order.
and EN 13501-1. All metal components can be recycled (as scrap).
All plastic components have a high calorific value and
Fire protection can be sent for thermal recycling.
Name Value In countries where no thermal recycling or substance
Building material class - recycling is established, disposal takes place via the
Burning droplets - waste incineration plant.
Smoke gas development -
2.16 Further information
Water Additional information about our products can be found
at https://www.hansgrohe.com.
3. LCA: Calculation rules
3.1 Declared Unit processes in Germany. Green electricity from
The results of this EPD are valid for the following hydropower and wind power (50% each) is used for
functional unit: the French production site. US electricity mix is used
Provide sanitary function for one (1) average basic set for the US production site.
unit used in accordance with the manufacturer's Module A4:
recommendations for a 20-year life, following the All distribution transports to the customers were
manufacturer's operating instructions. An average considered.
conditioned basic set is considered the baseline flow. Module A5:
This module covers the installation process with the
Weighted averaging based on production tonnages in corresponding packaging waste generated that needs
2020 is chosen as basis for creating the environmental to be disposed.
profile. 80 different basic sets were considered. Module B1-B7:
These modules were considered, but evaluated as not
Functional unit relevant for the products and considered as zero.
Name Value Unit Modules C1-C4:
Declared unit 1 pce. The modules include the environmental impacts for
Functional unit 1 pce. dismantling of the products and the treatment of the
Functional unit with packaging 1.42 kg waste fractions until the end-of-waste status (EoW) is
Packaging 0.24 kg reached, including the associated transports at the end
Weight range of the products of the product life cycle.
0.33 - 7.86 kg
examined Module D:
Identification of the benefits and costs of the product
outside the system boundary. For waste, paper and
plastics, these consist of energy credits from thermal
utilization (A3, A5 and C3) in the form of the average
3.2 System boundary European electricity mix or thermal energy from natural
This representative EPD follows the EPD type "cradle gas. Recycling of paper, plastic and metal scrap
to gate - with options". The following life cycle modules results in credits of the respective raw materials for the
are declared: primary material portion of the input. The loads of the
Modules A1-A3: waste incineration and recycling processes are
The product stage begins with considering the assigned to the respective modules (A3, A5 and C3)
production of the necessary raw materials and and not to module D.
energies, including all corresponding upstream chains
and the actual procurement transports. Furthermore, 3.3 Estimates and assumptions
the entire manufacturing phase was mapped, including Energy and water consumption, material amount for
the treatment of production waste until the end-of- coating as well as waste during production could only
waste status (EoW) was reached. Green electricity be determined on concrete, existing products and not
from hydropower is used for the manufacturing on the average product. The highest value of all inputs
4 Environmental Product Declaration Hansgrohe Group – Basic Sets
and outputs for energy, waste and coating of the top 3.8 Allocation
seller, the lightest and the heaviest product was used For the production process nearly all raw materials,
for the calculation of energy, water, waste and coating. precursors and supplies could be assigned to the
For the incineration with energy recovery (thermal and declared product. Energy, water, galvanization process
electric) of waste, an r1 value of > 0.6 is assumed. The and production waste were assigned to the highest
net efficiency for the average waste incinerated is value of either the heaviest, lightest or most sold
between 38 % and 44 %, depending on the type of product of the product group. No byproducts are
waste respectively the disposal data set. produced and no allocation is required.
Some of the brass losses from brass processing in
3.4 Cut-off criteria module A3 are directly reused by Hansgrohe and are
The effect associated with the neglected mass shares modelled as a closed loop. Another part of the brass
is less than 5% of the effect categories per module. losses (brass particles and dusts) is disposed of as
The minimum limit of 1% total mass and the use of waste (without debits and credits).
renewable and nonrenewable primary energy is not Credits for plastics, paper and cardboard recycled in
exceeded. A5 and metallurgical waste in C3 are credited in
module D.
3.5 Background data Credits for the energy recovery of incinerated
The LCA software GaBi 10.6 was used to model the production waste in A1-3, paper, cardboard and
life cycle. The entire manufacturing process, as well as plastics in A5 and plastics and other materials in C3
energy consumption, were modelled on the basis of are credited in module D.
manufacturer specific data. The loads for waste water treatment and waste
However, generic background datasets were used for disposal of core sand, waste oil and hazardous waste
the upstream and downstream processes. The majority from the manufacturing phase are allocated to module
of the background datasets used were taken from the A3.
current version (2021.2) of Packaging:
the GaBi database. Ecoinvent Version 3.6 (2019) For paper and cardboard, recycling (91 %) and energy
datasets were only used when suitable GaBi datasets recovery (9 %) are considered on a pro rata basis. For
were not available. plastic, a proportionate recycling (52 %), energy
recovery (48 %) considered, based on Eurostat.
3.6 Data quality Deconstructed product at the end of life:
The background datasets used for accounting Since the product is predominantly made of metal, it is
purposes mainly originate from the respective updated assumed that most of its metallic components are
GaBi databases at the time of calculation. The data for recycled. 95 % of the non-metallic components are
the examined products was captured on incinerated with energy recovery and 5 % are disposed
the basis of evaluations of internal production and in landfill. For the metal components, it is assumed that
environmental data, the collection of LCA relevant data 90 % are sent for material recycling, 5 % for
within the supply chain, as well as the evaluation of incineration with energy recovery (C3) and 5 % are
relevant data for the energy supply. The collected disposed in landfill (C4).
data were checked for plausibility and consistency.
Good representativity can be assumed. 3.9 Comparability
Basically, a comparison or an evaluation of EPD data
For the assessment of the variability of the results, all is only possible if all the data sets to be compared
products were balanced in addition to the average were created according to EN 15804 and the building
product. See at chapter 6 for explanation of the context, respectively the product-specific
variability. characteristics of performance, are taken into account.
3.7 Period under review The background database used is GaBi 10.6 in the
Life cycle assessment data were collected in 2020. database version 2021.2
4. LCA: Scenarios and additional technical information
Characteristic product properties Transport distance (Truck) 626 km
Information on biogenic carbon Capacity utilisation (including
55 %
empty runs) (Truck)
Transport distance (Container
4570 km
Information on describing the biogenic Carbon Ship)
Content at factory gate Capacity utilisation (Container
80 %
The biogenic carbon content was calculated based on Ship)
the factors from the Thünen Intitute.
Name Value Unit Installation into the building (A5)
Biogenic carbon content in 0.097 kg C For the installation are required screws, glue, dowels,
accompanying packaging silicone, teflon tape and electricity for a drilling
machine. The packaging is disposed either by
recycling or incineration.
The following technical information is a basis for the Name Value Unit
declared modules. Packaging (Paper, cardboard and
0.243 kg
plastic)
Transport to the building site (A4) Electricity consumption 0.004 kWh
Name Value Unit Screws 0.02 kg
5 Environmental Product Declaration Hansgrohe Group – Basic Sets
Glue 0.1 kg
Dowels 0.01 kg
Silicone 0.02 kg
Teflon tape 0.1 m
End of life (C1-C4)
Name Value Unit
Collected separately 1.175 kg
Recycling 0.802 kg
Energy recovery 0.314 kg
Landfilling 0.059 kg
Reuse, recovery and/or recycling potentials (D),
relevant scenario information
The energy generated from energy recovery as well as
recycled materials are assigned to module D as
possible potentials or avoided loads in subsequent
systems. Credits are only given for the primary portion
of the inputs.
6 Environmental Product Declaration Hansgrohe Group – Basic Sets
5. LCA: Results
The following table shows the result of the LCA for 1 piece of an average basic set.
DESCRIPTION OF THE SYSTEM BOUNDARY (X = INCLUDED IN LCA; ND = MODULE OR INDICATOR NOT
DECLARED; MNR = MODULE NOT RELEVANT)
BENEFITS AND
CONSTRUCTI LOADS
PRODUCT STAGE ON PROCESS USE STAGE END OF LIFE STAGE BEYOND THE
STAGE SYSTEM
BOUNDARIES
7 Environmental Product Declaration Hansgrohe Group – Basic Sets
lairetam
waR
ylppus tropsnarT
gnirutcafunaM
eht
morf
tropsnarT
etis
eht
ot
etag
ylbmessA esU
ecnanetniaM
riapeR
tnemecalpeR tnemhsibrufeR
ygrene
lanoitarepO esu
retaw
lanoitarepO esu
noitcurtsnoc-eD
noitilomed tropsnarT
gnissecorp
etsaW
lasopsiD -esueR -yrevoceR -gnilcyceR laitnetop
A1 A2 A3 A4 A5 B1 B2 B3 B4 B5 B6 B7 C1 C2 C3 C4 D
X X X X X X X X X X X X X X X X X
RESULTS OF THE LCA - ENVIRONMENTAL IMPACT according to EN 15804+A2: 1 piece average basic set
incl. packaging
Core Indicator Unit A1-A3 A4 A5 B1 B2 B3 B4 B5 B6 B7 C1 C2 C3 C4 D
2.20E+ 0.00E+ 0.00E+ 0.00E+ 0.00E+ 0.00E+ 0.00E+ 0.00E+ 0.00E+ -7.48E-
GWP-total [kg CO2-Eq.]
0
1.31E-16.24E-1
0 0 0 0 0 0 0 0
2.00E-26.11E-13.17E-3
1
2.55E+ 0.00E+ 0.00E+ 0.00E+ 0.00E+ 0.00E+ 0.00E+ 0.00E+ 0.00E+ -3.98E-
GWP-fossil [kg CO2-Eq.]
0
1.30E-12.70E-1
0 0 0 0 0 0 0 0
1.98E-26.11E-13.17E-3
1
-3.54E- 0.00E+ 0.00E+ 0.00E+ 0.00E+ 0.00E+ 0.00E+ 0.00E+ 0.00E+ 0.00E+ 0.00E+ 0.00E+ 0.00E+ -3.49E-
GWP-biogenic [kg CO2-Eq.]
1 0
3.54E-1
0 0 0 0 0 0 0 0 0 0 0 1
0.00E+ 0.00E+ 0.00E+ 0.00E+ 0.00E+ 0.00E+ 0.00E+ 0.00E+ -1.28E-
GWP-luluc [kg CO2-Eq.] 6.13E-36.18E-43.43E-4
0 0 0 0 0 0 0 0
1.63E-46.02E-53.02E-6
3
2.05E- 1.97E- 0.00E+ 0.00E+ 0.00E+ 0.00E+ 0.00E+ 0.00E+ 0.00E+ 0.00E+ 3.93E- 6.93E- 7.51E- -6.07E-
ODP [kg CFC11-Eq.] 6.01E-9
17 15 0 0 0 0 0 0 0 0 18 11 18 9
0.00E+ 0.00E+ 0.00E+ 0.00E+ 0.00E+ 0.00E+ 0.00E+ 0.00E+ -4.80E-
AP [mol H+-Eq.] 1.61E-22.13E-31.02E-3 3.33E-53.82E-49.93E-6
0 0 0 0 0 0 0 0 3
0.00E+ 0.00E+ 0.00E+ 0.00E+ 0.00E+ 0.00E+ 0.00E+ 0.00E+ -1.56E-
EP-freshwater [kg P-Eq.] 1.86E-42.36E-74.23E-7 5.91E-81.00E-71.84E-7
0 0 0 0 0 0 0 0 4
0.00E+ 0.00E+ 0.00E+ 0.00E+ 0.00E+ 0.00E+ 0.00E+ 0.00E+ -6.40E-
EP-marine [kg N-Eq.] 2.39E-35.78E-41.79E-4 1.31E-51.76E-42.45E-6
0 0 0 0 0 0 0 0 4
0.00E+ 0.00E+ 0.00E+ 0.00E+ 0.00E+ 0.00E+ 0.00E+ 0.00E+ -7.10E-
EP-terrestrial [mol N-Eq.] 2.53E-26.36E-31.96E-3 1.50E-42.03E-32.65E-5
0 0 0 0 0 0 0 0 3
0.00E+ 0.00E+ 0.00E+ 0.00E+ 0.00E+ 0.00E+ 0.00E+ 0.00E+ -1.89E-
POCP [kg NMVOC-Eq.]7.07E-31.59E-36.00E-4 2.97E-54.53E-47.71E-6
0 0 0 0 0 0 0 0 3
0.00E+ 0.00E+ 0.00E+ 0.00E+ 0.00E+ 0.00E+ 0.00E+ 0.00E+ 2.18E- -3.43E-
ADPE [kg Sb-Eq.] 7.15E-48.32E-95.69E-6 1.76E-99.60E-9
0 0 0 0 0 0 0 0 10 4
-
4.65E+ 1.66E+ 4.54E+ 0.00E+ 0.00E+ 0.00E+ 0.00E+ 0.00E+ 0.00E+ 0.00E+ 0.00E+
ADPF [MJ] 2.65E-14.55E-14.59E-24.64E+
1 0 0 0 0 0 0 0 0 0 0
0
[m³ world-Eq 1.27E+ 0.00E+ 0.00E+ 0.00E+ 0.00E+ 0.00E+ 0.00E+ 0.00E+ 0.00E+ -3.57E- -7.77E-
WDP 7.83E-46.59E-2 1.85E-46.91E-2
deprived] 0 0 0 0 0 0 0 0 0 5 1
GWP = Global warming potential; ODP = Depletion potential of the stratospheric ozone layer; AP = Acidification potential of land and water; EP =
Caption Eutrophication potential; POCP = Formation potential of tropospheric ozone photochemical oxidants; ADPE = Abiotic depletion potential for non-
fossil resources; ADPF = Abiotic depletion potential for fossil resources; WDP = Water (user) deprivation potential
RESULTS OF THE LCA - INDICATORS TO DESCRIBE RESOURCE USE according to EN 15804+A2: 1 piece
average basic set incl. packaging
Indicator Unit A1-A3 A4 A5 B1 B2 B3 B4 B5 B6 B7 C1 C2 C3 C4 D
PERE [MJ] 6.33E+0 6.01E-2 5.31E+00.00E+00.00E+00.00E+00.00E+00.00E+00.00E+00.00E+00.00E+0 1.53E-2 1.89E-1 3.33E-3-1.76E+0
PERM [MJ] 3.97E+00.00E+0-3.97E+00.00E+00.00E+00.00E+00.00E+00.00E+00.00E+00.00E+00.00E+00.00E+00.00E+00.00E+00.00E+0
PERT [MJ] 1.03E+1 6.01E-2 1.34E+00.00E+00.00E+00.00E+00.00E+00.00E+00.00E+00.00E+00.00E+0 1.53E-2 1.89E-1 3.33E-3-1.76E+0
PENRE [MJ] 3.62E+11.67E+04.70E+00.00E+00.00E+00.00E+00.00E+00.00E+00.00E+00.00E+00.00E+0 2.66E-1 1.01E+1 4.59E-2-4.64E+0
PENRM [MJ] 1.03E+10.00E+0-1.56E-10.00E+00.00E+00.00E+00.00E+00.00E+00.00E+00.00E+00.00E+00.00E+0-9.68E+00.00E+00.00E+0
PENRT [MJ] 4.65E+11.67E+04.54E+00.00E+00.00E+00.00E+00.00E+00.00E+00.00E+00.00E+00.00E+0 2.66E-1 4.55E-1 4.59E-2-4.64E+0
SM [kg] 1.05E+00.00E+00.00E+00.00E+00.00E+00.00E+00.00E+00.00E+00.00E+00.00E+00.00E+00.00E+00.00E+00.00E+0 1.28E-1
RSF [MJ] 0.00E+00.00E+00.00E+00.00E+00.00E+00.00E+00.00E+00.00E+00.00E+00.00E+00.00E+00.00E+00.00E+00.00E+00.00E+0
NRSF [MJ] 0.00E+00.00E+00.00E+00.00E+00.00E+00.00E+00.00E+00.00E+00.00E+00.00E+00.00E+00.00E+00.00E+00.00E+00.00E+0
FW [m³] 3.32E-2 6.99E-5 2.28E-3 0.00E+00.00E+00.00E+00.00E+00.00E+00.00E+00.00E+00.00E+0 1.75E-5 1.69E-3 5.12E-7-1.79E-2
PERE = Use of renewable primary energy excluding renewable primary energy resources used as raw materials; PERM = Use of
renewable primary energy resources used as raw materials; PERT = Total use of renewable primary energy resources; PENRE = Use of
non-renewable primary energy excluding non-renewable primary energy resources used as raw materials; PENRM = Use of non-
Caption
renewable primary energy resources used as raw materials; PENRT = Total use of non-renewable primary energy resources; SM = Use
of secondary material; RSF = Use of renewable secondary fuels; NRSF = Use of non-renewable secondary fuels; FW = Use of net fresh
water
RESULTS OF THE LCA – WASTE CATEGORIES AND OUTPUT FLOWS according to EN 15804+A2:
1 piece average basic set incl. packaging
Indicator Unit A1-A3 A4 A5 B1 B2 B3 B4 B5 B6 B7 C1 C2 C3 C4 D
HWD [kg] 6.69E-65.83E-112.60E-9 0.00E+00.00E+00.00E+00.00E+00.00E+00.00E+00.00E+00.00E+01.40E-111.29E-108.16E-12-7.23E-6
NHWD [kg] 2.37E-1 2.24E-4 4.28E-2 0.00E+00.00E+00.00E+00.00E+00.00E+00.00E+00.00E+00.00E+0 4.17E-5 2.72E-2 5.87E-2-8.18E-2
RWD [kg] 1.02E-3 2.56E-6 1.54E-4 0.00E+00.00E+00.00E+00.00E+00.00E+00.00E+00.00E+00.00E+0 4.83E-7 2.75E-5 5.26E-7-1.00E-4
CRU [kg] 0.00E+00.00E+00.00E+00.00E+00.00E+00.00E+00.00E+00.00E+00.00E+00.00E+00.00E+00.00E+00.00E+00.00E+00.00E+0
MFR [kg] 0.00E+00.00E+0 2.19E-1 0.00E+00.00E+00.00E+00.00E+00.00E+00.00E+00.00E+00.00E+00.00E+0 8.03E-1 0.00E+00.00E+0
MER [kg] 0.00E+00.00E+00.00E+00.00E+00.00E+00.00E+00.00E+00.00E+00.00E+00.00E+00.00E+00.00E+00.00E+00.00E+00.00E+0
EEE [MJ] 1.60E-2 0.00E+0 5.78E-2 0.00E+00.00E+00.00E+00.00E+00.00E+00.00E+00.00E+00.00E+00.00E+0 8.73E-3 8.76E-5 0.00E+0
EET [MJ] 3.17E-2 0.00E+0 1.04E-1 0.00E+00.00E+00.00E+00.00E+00.00E+00.00E+00.00E+00.00E+00.00E+0 1.64E-2 0.00E+00.00E+0
HWD = Hazardous waste disposed; NHWD = Non-hazardous waste disposed; RWD = Radioactive waste disposed; CRU = Components
Caption for re-use; MFR = Materials for recycling; MER = Materials for energy recovery; EEE = Exported electrical energy; EET = Exported
thermal energy
RESULTS OF THE LCA – additional impact categories according to EN 15804+A2-optional:
1 piece average basic set incl. packaging
Indicator Unit A1-A3 A4 A5 B1 B2 B3 B4 B5 B6 B7 C1 C2 C3 C4 D
[Disease 2.08E- 1.05E-
PM 1.41E-7 3.50E-8 1.45E-80.00E+00.00E+00.00E+00.00E+00.00E+00.00E+00.00E+00.00E+0 1.70E-9 -4.80E-8
Incidence] 10 10
[kBq U235-
IRP 1.74E-1 3.72E-4 2.33E-20.00E+00.00E+00.00E+00.00E+00.00E+00.00E+00.00E+00.00E+07.06E-5 2.83E-3 7.54E-5-3.19E-2
Eq.]
-
ETP-fw [CTUe] 7.21E+11.22E+01.73E+00.00E+00.00E+00.00E+00.00E+00.00E+00.00E+00.00E+00.00E+01.97E-1 2.75E-1 2.29E-2
2.51E+1
2.40E- 3.98E- 9.39E- 1.70E-
HTP-c [CTUh] 2.91E-8 3.17E-80.00E+00.00E+00.00E+00.00E+00.00E+00.00E+00.00E+00.00E+0 -1.53E-9
11 12 12 12
2.12E- 6.77E- 1.61E-
HTP-nc [CTUh] 9.69E-8 1.22E-9 8.62E-80.00E+00.00E+00.00E+00.00E+00.00E+00.00E+00.00E+00.00E+0 -2.71E-8
10 10 10
-
SQP [-] 2.05E+13.47E-14.87E+00.00E+00.00E+00.00E+00.00E+00.00E+00.00E+00.00E+00.00E+09.11E-2 1.62E-1 3.32E-3
7.22E+0
PM = Potential incidence of disease due to PM emissions; IR = Potential Human exposure efficiency relative to U235; ETP-fw = Potential
Caption comparative Toxic Unit for ecosystems; HTP-c = Potential comparative Toxic Unit for humans (cancerogenic); HTP-nc = Potential
comparative Toxic Unit for humans (not cancerogenic); SQP = Potential soil quality index
Disclaimer 1 – for the indicator “Potential Human exposure efficiency relative to U235”.
This impact category deals mainly with the eventual impact of low dose ionizing
radiation on human health of the nuclear fuel cycle. It does not consider effects due to possible
nuclear accidents, occupational exposure nor due to radioactive waste disposal in underground
facilities. Potential ionizing radiation from the soil, from radon and from some construction materials is also not
measured by this indicator.
Disclaimer 2 – for the indicators “abiotic depletion potential for non-fossil resources”, “abiotic depletion potential
for fossil resources”, “water (user) deprivation potential, deprivation-weighted water consumption”, “potential
comparative toxic unit for ecosystems”, “potential comparative toxic unit for humans – cancerogenic”, “Potential
comparative toxic unit for humans - not cancerogenic”, “potential soil quality index”.
The results of this environmental impact indicator shall be used with care as the
uncertainties on these results are high or as there is limited experienced with the indicator.
6. LCA: Interpretation
8 Environmental Product Declaration Hansgrohe Group – Basic Sets
The dominance analysis shows that module A1-A3 in results, all products were balanced and compared to
particular is the dominant life cycle stage in regard to the average product weighted by production volume.
GWPtotal (2.20 kg CO2-eq.). This is mainly caused by The different types of products all have the same
the provision of brass for the production of the basic function and differ mainly in terms of design, which has
sets at the production site (0.64 kg CO2-eq.) an influence on construction and materials used. The
The end-of-life stage (module C1-C4) has a basic structure of the product types is always similar.
noteworthy influence on the indicator GWPtotal and Material type and quantity proportions do not differ
also on AP, EP, POCP and WDP. Here, these much, as also shown in the average material
indicators are each influenced primarily by the thermal composition table.
treatment of plastics. 92% of the produced basic sets are close to or below
The environmental burden from the transport (module the average value of GWP fossil. The products with
A4) has a noticeable impact on GWPluluc, AP, deviations higher than the average product are only
EPmarine, EPterrestrial and POCP. produced in smaller quantities (8% of total production).
The possible potentials of avoided loads of subsequent The maximum deviation is 518% and the minimum
systems (module D) lie outside the considered system deviation is -68%. All top sellers are below the
boundaries and relate exclusively to credits from average.
recycling and thermal recycling by means of The deviation correlates in general with the weight of
incineration with energy recovery of the different the product. However, also the material composition
materials. does play a role in the variability. This is caused by the
954,358 basic sets of 80 different product types were ratio of metal and plastic. The products with a higher
produced. For the assessment of the variability of the plastic content cause a higher GWP impact in the end
of life because they are incinerated instead of recycled.
7. Requisite evidence
The drinking water regulation determines the quality of  Metal recommendation of the federal
drinking water at the point of withdrawal. This result in environment agency: metal materials suitable
requirements for used materials in drinking water
for drinking water hygiene
installations in general and therefore in sanitary fittings
in particular.
All materials used by Hansgrohe SE, which are in Regulations for other materials (Germany):
contact with drinking water, fulfill the drinking water  KTW: Assessment basis for plastics and other
regulation. organic materials in contact with drinking
Regulations for metals (Europe-wide): water
 Acceptance of metallic materials used for
 Elastomer guideline: Guideline for the
products in contact with drinking water: 4MS
hygienic assessment of elastomers in contact
Common Approach
with drinking water
 Thermoplastic elastomers: Recommendation
- Part A – Procedure for the acceptance for the hygienic assessment of products made
- Part B – 4MS Common Composition List
of thermoplastic elastomers in contact with
drinking water (TPE transition
recommendation)
9 Environmental Product Declaration Hansgrohe Group – Basic Sets
 Ceramics: draft assessment basis for  ACS: Attestation de Conformité Sanitaire
enamels and ceramic materials: assessment (plastics, elastomers, metals)
basis for enamels and ceramic materials in
contact with drinking water (enamel/ceramic Regulation for other materials (UK):
assessment basis)  BS 69 20: Suitability of non-metallic products
 Lubricants: Guideline for the hygienic for use in contact with water intended for
assessment of lubricants in contact with human consumption with regard to their effect
drinking water (sanitary lubricants), (Lubricant on the quality of water (plastics, elastomers)
Guideline)
Products of the Hansgrohe SE are therefore uncritical
Regulation for other materials (France): to use with any drinking water.
8. References
Standards safety management systems — Requirements with
guidance for use. 2018-03
EN 200
EN 200:2008: Sanitary tapware – Single taps and DIN EN ISO 50001
combination taps for water supply systems of type 1 DIN EN ISO 50001:2018: Energy management
and type 2 systems — Requirements with guidance for use. 2018-
08
EN 816
EN 816:2017: Sanitary tapware – Automatic shut-off Further References
valves PN 10
AVV
EN 817 Draft General administrative provision relating to the
EN 817:2008: Sanitary tapware – Mechanical mixing Order on the European list of wastes (Waste List Order
valves (PN 10) – German designation: AVV) of 10 December 2001.
ISO 3822 ECHA
ISO 3822: Acoustics – Laboratory tests on noise European Chemicals Agency (ECHA) Candidate List of
emission from appliances and equipment used in water Substances of Very High Concern (SVHC) for
supply installations Authorisation https://echa.europa.eu/de/candidate-
listtable
DIN 4102-1
DIN 4102-1: Fire behaviour of building materials and Ecoinvent
building components - Part 1: Building materials; ecoinvent 3.6 Database on Life Cycle Inventories (Life
concepts, requirements and tests. 1998-05 Cycle Inventory data), ecoinvent Association, Zürich,
2020
DIN EN ISO 9001
DIN EN ISO 9001:2015: Quality management systems EU Ordinance on biocide Products No. 528/2012
- Requirements (ISO 9001:2015) European Parliament, 2012. Regulation (EU) no
528/2012 of the European parliament and of the
DIN EN 13501-1 council of 22 May 2012 concerning the making
DIN EN 13501-1:2019-05: Fire classification of available on the market and use of biocidal products
construction products and building elements - Part 1:
Classification using data from reaction to fire tests; Eurostat
German version EN 13501-1:2018 Eurostat, last update 26/10/2021 on
https://ec.europa.eu/eurostat/databrowser/view/ten000
DIN EN ISO 14001 63/default/table?lang=en
DIN EN ISO 14001:2015, Environmental management
systems — Requirements with guidance for use, 2015- GaBi
09 GaBi 10.6, GaBi Software System and Database for
Life Cycle Engineering version 2021.2, Sphera
DIN EN ISO 14025 Solutions GmbH, Leinfelden-Echterdingen, 1992-2021
DIN EN ISO 14025: Environmental labels and
declarations - Type III environmental declarations - IBU 2021
Principles and procedures, 2011-10 General Instructions for the EPD programme of Institut
Bauen und Umwelt e.V. Version 2.0, Berlin: Institut
EN 15804 Bauen und Umwelt e.V., 2021, www.ibu-epd.com
DIN EN 15804:2012+A2:2019+AC:2021: Sustainability
of construction works - Environmental product PCR Part A
declarations - Core rules for the product category of Institut Bauen und Umwelt e.V. (IBU), Product
construction products Category Rules for Building-Related Products and
Services. Part A: Calculation rules for the life cycle
DIN EN ISO 45001 assessment and requirements on the project report.
DIN EN ISO 45001:2018: Occupational health and Version 2.1, Berlin, 11/2021
10 Environmental Product Declaration Hansgrohe Group – Basic Sets
Diestel, Sylvia / Weimar, Holger: Der Kohlenstoffgehalt
PCR Part B in Holz- und Papierprodukten - Herleitung und
Institut Bauen und Umwelt e.V. (IBU), Requirements Umrechnungsfaktoren. Thünen Working Paper 38.
on the EPD for fittings and showers. Version 1.1, Johann Heinrich von Thünen-Institut. Hamburg, 2014
Berlin, 03/2022
Thünen Institute
11 Environmental Product Declaration Hansgrohe Group – Basic Sets
Publisher
Institut Bauen und Umwelt e.V. Tel +49 (0)30 3087748- 0
Hegelplatz 1 Fax +49 (0)30 3087748- 29
10117 Berlin Mail info@ibu-epd.com
Germany Web www.ibu-epd.com
Programme holder
Institut Bauen und Umwelt e.V. Tel +49 (0)30 - 3087748- 0
Hegelplatz 1 Fax +49 (0)30 – 3087748 - 29
10117 Berlin Mail info@ibu-epd.com
Germany Web www.ibu-epd.com
Author of the Life Cycle
Assessment Tel +49 421 70 90 84 33
brands & values GmbH Fax +49 421 70 90 84 35
Altenwall 14 Mail info@brandsandvalues.com
28195 Bremen Web www.brandsandvalues.com
Germany
Owner of the Declaration
Hansgrohe Group Tel +49 7836 51-0
Auestr. 5-9 Fax +49 7836 51-1300
77761 Schiltach Mail info@hansgrohe-group.com
Germany Web http://www.hansgrohe-
group.com
