ENVIRONMENTAL PRODUCT DECLARATION
as per ISO 14025 and EN 15804+A2
Owner of the Declaration Knauf Ceiling Solutions GmbH & Co. KG
Publisher Institut Bauen und Umwelt e.V. (IBU)
Programme holder Institut Bauen und Umwelt e.V. (IBU)
Declaration number EPD-KNA-20240463-IBA1-EN
Issue date 06.12.2024
Valid to 05.12.2029
Heradesign Corridor Fine
Knauf Ceiling Solutions GmbH & Co. KG
www.ibu-epd.com | https://epd-online.com
1. General Information
Knauf Ceiling Solutions GmbH & Co. KG Heradesign Corridor Fine
Programme holder Owner of the declaration
IBU – Institut Bauen und Umwelt e.V. Knauf Ceiling Solutions GmbH & Co. KG
Hegelplatz 1 Elsenthal 15
10117 Berlin 94481 Grafenau
Germany Germany
Declaration number Declared product / declared unit
EPD-KNA-20240463-IBA1-EN 1 m² Heradesign Corridor Fine (Euroclass B).
This declaration is based on the product category rules: Scope:
Wood cement - Mineral-bonded wooden composites, 01.08.2021 This document refers to 1 m² of Heradesign Corridor Fine (Euroclass B)
(PCR checked and approved by the SVR) with a surface weight of 13.3 kg/m² manufactured at the production facility
in Ferndorf (Austria). The product is a magnesite bonded wood wool panel.
Issue date The owner of the declaration shall be liable for the underlying information
and evidence; the IBU shall not be liable with respect to manufacturer
06.12.2024
information, life cycle assessment data and evidences.
The EPD was created according to the specifications of EN 15804+A2. In
Valid to
the following, the standard will be simplified as EN 15804.
05.12.2029
Verification
The standard EN 15804 serves as the core PCR
Independent verification of the declaration and data according to ISO
14025:2011
internally X externally
Dipl.-Ing. Hans Peters
(Chairman of Institut Bauen und Umwelt e.V.)
Florian Pronold Matthias Schulz,
(Managing Director Institut Bauen und Umwelt e.V.) (Independent verifier)
1 Environmental Product Declaration - Knauf Ceiling Solutions GmbH & Co. KG - Heradesign Corridor Fine
2. Product
The products are delivered packed in cardboard on pallets.
2.1 Product description/Product definition
Heradesign panels are wood wool panels in accordance with 2.5 Base materials/Ancillary materials
EN 13168 and/or EN 13964, manufactured from wood wool and
Composition of HERADESIGN products:
mineral binding agents.
Name Value Unit
Product name: 34 (+/-
Spruce (Picea abies) (structural material) %
3)
HERADESIGN Corridor Fine 50 (+/-
Anorganic binder %
3)
For the marketing of the products in the European Magnesium sulphate (MgSO4) CAS: 7487-88-9
5 (+/- 1) %
Union/European Free Trade Association (EU/EFTA) (with the (co-binding partner)
exception of Switzerland) Regulation (EU) No. 305/2011 (CPR)
Water (H2O) CAS: 7732-16-5 (solvent for 11 (+/-
applies. %
magnesium sulphate) 3)
The products require a declaration of performance taking into
account EN 13168:2012+A1:2015, Thermal insulation products The spruce wood is procured from sustainable forest
for buildings - Factory made wood wool (WW) products - management and serves as a substrate. Caustic magnesia is
Specification or EN 13964:2014, Suspended ceilings - extracted from regional magnesite raw material. Magnesium
Requirements and test methods and the CE marking. sulphate serves as a co-binding partner; water is partially
The respective national regulations apply to their use. bound in the form of crystal water and partially contained as
residual moisture. No biocides or fire retardants are used in the
2.2 Application product.
Heradesign acoustic panels are primarily used as For optical reasons, the finished products are dyed on the
acoustic/decorative wall and ceiling panelling in offices, visible side using dispersion paint.
kindergartens etc.
At least one sub-product contains substances of the candidate
2.3 Technical Data list (date 27.06.2024) above 0.1 % by mass: no.
Product-specific values can be found at
http://www.knaufceilingsolutions.com The product contains other cancerogenic, mutagenic,
Constructional data reprotoxic (CMR) substances of category 1A or 1B that are not
on the candidate list, above 0,1 % by mass in at least one part
Name Value Unit
product: no.
Gross density acc. to EN 1602 532 kg/m3
Grammage 13,3 kg/m2 Biocidal products have been added to this construction product
Thickness 25 mm or it has been treated with biocidal products (it is therefore a
treated product within the meaning of the Biocidal Products
Bending strength (longitudinal) n.r. N/mm2
Regulation (EU) No 528/2012): no.
Bending strength (transverse) n.r. N/mm2
E-module (longitudinal) n.r. N/mm2 No fire retardants were used in the product.
E-module (transverse) n.r. N/mm2
2.6 Manufacture
Tensile strength rectangular n.r. N/mm2 2.6.1 Raw material
Thermal conductivity acc. to EN 12667 0.11 W/(mK) Spruce wood is stored as trunks 2 metres in length. Depending
Water vapour diffusion resistance factor acc. on climate conditions, storage lasts around 6-12 months. The
to DIN 4108-4 2 - 5 - trunks are transported by conveyor belts to a multi-rip saw, cut
into pieces and processed as wood wool using a planing
Moisture content at 23 °C, 80% 11 M.-%
machine. The binding agent components are stored in steel
Coefficient of thermal expansion n.r. 10-6K-1
silos.
Swelling (air-dry to water-saturated) n.r. %
Sound absorption coefficient (only with up to 2.6.2 Mixer
%
reference to component design) 0.95 Wood wool, as well as a binding agent and a magnesium
sulphate solution, are required for generating a mixture for
n.r. = not relevant
wood wool pellets. These components are transported to a
mixer where they are processed to form the requisite formula.
Performance data of the product in accordance with the
declaration of performance with respect to its essential
2.6.3 Scattering and shaping
characteristics to EN 13168:2012+A1:2015, Thermal insulation
The mixture is scattered onto a steel band and passed through
products for buildings - Factory made wood wool (WW)
a binding channel, whereby it is separated from the room by a
products - Specification or rather EN 13964:2014, Suspended
second horizontal steel strip as well as two side strips. An
ceilings - Requirements and test methods.
endless product is produced on leaving the twin belt. The raw
2.4 Delivery status goods are then cut to the desired length.
Wood wool products are exclusively available as panels.
Typical dimensions:
Lengths: max. 2400 mm and on request
Widths: 600 mm
Thicknesses: 25 mm
2 Environmental Product Declaration - Knauf Ceiling Solutions GmbH & Co. KG - Heradesign Corridor Fine
2.9 Packaging
Heradesign acoustic panels are supplied in protective
cardboard packaging with polypropylene (PP) straps on
untreated wooden pallets. It must be ensured that the
packaging materials are separated and disposed of where such
waste incurs.
2.10 Condition of use
No emissions are to be expected during the use phase of the
Heradesign acoustic panels because the ingredients are firmly
2.6.4 Interim storage and picking bound in the state of use.
The products are put into interim storage for 3-5 days (drying Heradesign acoustic panels do not require any maintenance
and maturing process). The requisite edge design is then from which significant effects on the environment can be
produced on so-called double-end profiling machines. expected.
Edge processing: 18 standard edges are possible. Cleaning is done by sweeping off occasionally. No effects are
assumed in Module B3 (Repair) because the repair of
Heradesign acoustic panels is rarely necessary. In the case of a
repair, the entire board is replaced, which would correspond to
the environmental impact declared in modules A1–A3.
No effects are assumed for modules B4 and B5 either, because
with Heradesign acoustic panels, when used as intended, no
replacement or renewal is required during the service life of 50
years. Modules B6 (energy use for operating the building) and
B7 (water use for operating the building) are not relevant for
Heradesign acoustic panels.
2.6.5 Dyeing, packaging and shipping
The requisite colour is applied in a dyeing plant, followed by 2.11 Environment and health during use
packaging and storage. According to current knowledge, hazards to water, air and soil
Dyeing: Possible in many RAL colours (left) Products ready for cannot arise if the described products are used as intended.
storage (right) Heradesign products meet the requirements of the Blue Angel
(RAL UZ 132, low-emission thermal insulation materials and
suspended ceilings for use in buildings, October 2010) and the
Danish Indoor Climate label. Test reports from eurofins confirm
the fulfilment of the requirements for building structures with
regard to health protection (ABG), draft 31.08.2017, as well as
the achievement of class A+ of the French Volatile Organic
Compound (VOC) regulation (regulation March and April 2011
(DEVL1101903D and DECL1104875A)).
2.12 Reference service life
The service life of Heradesign products is 50 years, but it
depends mainly on the life of the building. Due to the mineral
2.7 Environment and health during manufacturing
binder, no ageing processes are known.
The Ferndorf manufacturing plant places great value on the
Employee safety and has a security management system 2.13 Extraordinary effects
according to ISO 45001. In addition to the compliance with the
Fire
environmental requirements of the authorities the
Reaction to fire: Class B-, s1-, d0 nach EN 13501-1
manufacturing plant operates an environmental management
Reaction to fire:
system according to ISO 14001 and energy management
according to ISO 50001 to keep the environmental impact as Name Value
low as possible. Building material class nach EN 13501-1 B
Burning droplets nach EN 13501-1 d0
The Bureau Veritas certificate confirms compliance with the
Smoke gas development nach EN 13501-1 s1
specified requirements. The manufacturing plant has a "zero
waste policy", all production-related waste (cutting waste,
production residues) is returned to the production process in Water
the course of raw material preparation. Heradesign acoustic panels are intended for indoor use. Should
This also applies to washing water, which is also 100 % an unforeseen water effect, e.g. a flood, occur, the panels are
recycled in the production process. fully functional again after drying. There is no impairment of the
environment to be expected.
2.8 Product processing/Installation
The type of mounting is described in detail in the brochure
"System solutions". In it, the possible systems, concealed Mechanical destruction
systems, screw systems etc. are dealt with in detail. This point is not relevant for a wood-wool building board, as
For further information, in addition to the "System Solutions" there is no environmental impact in case of unforeseen
brochure, individual processing videos can also be downloaded destruction. It would be more an optical defect.
from the website www.knaufceilingsolutions.com.
2.14 Re-use phase
Uncontaminated Heradesign panels can be reused. The
following reuse options are available:
3 Environmental Product Declaration - Knauf Ceiling Solutions GmbH & Co. KG - Heradesign Corridor Fine
Re-use: slabs from demolition activities can easily be disposed of in
Clean Heradesign panels can be re-used. landfills without pretreatment due to their predominantly mineral
By screw mounting or an inserted T-rail, re- and new mounting content.
is easily possible without damaging the product. Waste code EAK-code: 17 01 07
Composting: Thermal recycling:
Wood wool panels, mechanically shredded, can be converted In the manufacturing plant, waste plates can be recycled to
into compost material by enrichment with appropriate bacteria. binder in a rotary kiln process. This would be the preferred way
This material can then be used for soil improvement in in terms of a functioning recycling economy.
agriculture.
2.16 Further information
2.15 Disposal Further information, for example, product data sheets, safety
If the above-mentioned recycling options are not practicable, data sheets or declarations of performances are available on
the slab residues arising on the construction site as well as the website www.knaufceilingsolutions.com.
3. LCA: Calculation rules
Module C3 | Waste processing
3.1 Declared Unit The declared scenario assumes landfilling of the product.
This EPD refers to a declared unit of 1 m² of Heradesign Referring environmental impacts are accounted for in module
Corridor Fine (Euroclass B). The declared unit refers to a C4. Therefore, no environmental impacts from waste
surface weight of 13.3 kg/m². processing of the product are expected in C3.
Declared unit
Module C4 | Disposal
Name Value Unit
Modul C4 declares the environmental impacts from landfilling
Declared unit 1 m²
after use of the product. The biogenic carbon in the wood share
Grammage 13.3 kg/m2 of the product is treated as emissions of biogenic CO from the
2
Grammage 0.013 t/m² technosphere to the natural environment.
Conversion factor to 1 t 75.19 m²/t
Module D | Benefits and loads beyond the system
Layer thickness 0.025 m
boundary
Other declared units are allowed if the conversion is shown The declared scenario assumes landfilling of the product.
transparently. Referring environmental impacts are accounted for in module
C4. No benefits or loads outside the system boundary in
Various Heradesign products are manufactured at the site. The Module D are to be expected.
allocation of product specific material and energy flows for the
different Euroclasses produced (B and A2) is based on the 3.3 Estimates and assumptions
composition of the referring products. All assumptions are verified through detailed documentation
and correspond to the best possible representation of reality
3.2 System boundary
based on the available data. Regional applicability of the used
The life cycle assessment of Heradesign ceiling panels includes background data refers to average data under European or
a cradle-to-gate analysis of the environmental impacts with German conditions taken from the GaBi database. German
modules C1–C4 and module D (A1–A3, + C + D). Subsequent data were used for the Austrian market whenever European or
life cycle phases are part of the analysis: regionalised average data were not available.
Module A1–A3 | Production stage 3.4 Cut-off criteria
The production stage includes upstream burdens of raw All inputs and outputs for which data are available and a
materials (wood, binding agents, recalcination, auxiliaries, etc.) significant impact is expected are included in the LCA model.
and the corresponding transports to the production site in Data gaps are filled with conservative assumptions from
Ferndorf (Austria). Material and energy flows needed for the average data (when available) or with generic data and are
mixing of the components, scattering and shaping, interim documented accordingly. Only data with a contribution of less
storage and picking as well as dyeing and packaging were than 1 % were cut off. Ignoring such data is justified based on
specifically recorded. In addition, the recalcination process for the insignificance of the expected effect. Processes, materials
the provision of Knauf Sekundärkauster is considered. The or emissions known to have a significant contribution to the
representation of all specific input and output flows is thus environmental effects of the products under examination have
based on company-specific foreground data. 100 % green not been neglected. The data collection was verified using
electricity is used in the production. Thermal energy results available comparative values. It is assumed that the data have
from energy recovery from the recalcination process been completely recorded and that the overall total of ignored
supplemented by natural gas. input flows does not amount to more than 5 % of the total
Module C1 | Deconstruction and demolition energy and mass flows. Environmental impacts of machines,
Disassembly of the product is done either manually or using plant and infrastructure were not included.
smaller tools. Referring energy demand is considered to be
negligible. 3.5 Background data
This study uses generic background data for the evaluation of
Module C2 | Transport to disposal upstream environmental impacts from GaBi databases (GaBi
The transport to the disposal of the material is estimated 10; 2022.2).
declaring a 50 km radius to the landfill. In reality, this scenario
3.6 Data quality
may vary depending on the actual location of deconstruction
and referring waste treatment. Data collection is based on product-specific questionnaires. It
follows an iterative process clarifying questions via e-mail,
4 Environmental Product Declaration - Knauf Ceiling Solutions GmbH & Co. KG - Heradesign Corridor Fine
telephone calls or in personal or web-meetings. Intensive
discussions between Knauf Ceiling Solutions and Daxner & 3.9 Allocation
Merl results in an accurate mapping of product-related material The life cycle assessment considers the material inherent
and energy flows. This leads to a high quality of foreground properties of wood (carbon content and primary energy
data collected. Data collection relies on a consistent process content) and relies on its physical relations.
according to ISO 14044.
The annually used raw material and referring energy flows at
The technological, geographical and time-related Ferndorf were allocated to the specific products based on the
representativeness of the database was kept in mind when square meters produced yearly.
selecting background data. Whenever specific data were
missing, either generic datasets or representative average data Wooden residues result from the production process. As they
were used instead. The implemented GaBi background account for less than 1 % of the yearly turnover of the
datasets refer to the latest versions available (not more than organisation, they were not considered as co-products.
ten years old) and are carefully chosen. Referring quantities were cut-off.
3.7 Period under review 3.10 Comparability
Foreground data were collected in the 2018 production year, Basically, a comparison or an evaluation of EPD data is only
and the data are based on the volumes produced on an annual possible if all the data sets to be compared were created
basis. The data is representative for the production conditions according to EN 15804 and the building context, respectively
in 2022 at the site in Ferndorf. the product-specific characteristics of performance, are taken
into account.
3.8 Geographic Representativeness The GaBi background database was used to calculate the LCA
Land or region, in which the declared product system is (GaBi 10; 2022.2).
manufactured, used or handled at the end of the product´s
lifespan: Austria
4. LCA: Scenarios and additional technical information
Installation (A5)
Characteristic product properties of biogenic carbon
The End-of-Life of product packaging is not declared in module
The biogenic carbon content quantifies the amount of biogenic
A5.
carbon in the declared building product.
Name Value Unit
Production stage (A1–A3) Packaging (cardboard) 0.08 kg
In module A1–A3 the absorption of 6.92 kg biogenic CO 2 per Packaging (pallets) 0.21 kg
declared unit in the Heradesign ceiling panels has been
The biogenic carbon content of the cardboard and the wooden
considered, due to the carbon stored in the wood.
pallets has been treated CO -neutral and not accounted for as
In the recalcination process, the emissions of 0.81 kg of 2
biogenic CO were balanced in module A1–A3. carbon storage.
2
Information for describing the biogenic carbon content at
factory gate
End of Life (C1–C4)
Name ValueUnit
Name Value Unit
kg
Biogenic carbon content in product 1.89 Landfilling 13.3 kg
C
Biogenic carbon content in accompanying kg During landfilling 6.92 kg of biogenic CO 2 remain in the
0.13
packaging C product. Due to the binding properties of magnesite,
Heradesign ceiling panels can be deposited. This corresponds
Note: 1 kg of biogenic carbon is equivalent to 44/12 kg of CO .
2 to a representative scenario. Long-term landfill gas
measurements as well as periodic material withdrawals from
the deposited products confirm the retention of the biogenic
bound carbon during landfilling.
In accordance with the requirements of EN 15804+A2, the
biogenic carbon in the wood of the products is declared as
emissions of biogenic CO from the technosphere into the
2
natural environment in module C4.
5 Environmental Product Declaration - Knauf Ceiling Solutions GmbH & Co. KG - Heradesign Corridor Fine
5. LCA: Results
The following table contains the LCA results for a declared unit of 1 m² Heradesign Corridor Fine (Euroclass B) with a surface weight of
13.3 kg/m². This corresponds to 0.013 t/m².
DESCRIPTION OF THE SYSTEM BOUNDARY (X = INCLUDED IN LCA; MND = MODULE OR INDICATOR NOT DECLARED; MNR
= MODULE NOT RELEVANT)
Benefits and
Construction loads beyond
Product stage Use stage End of life stage
process stage the system
boundaries
la ire ta m w a Ry lp p u s tro p s n a rT g n iru tc a fu n a M e h t m o rf tro p s n a rTe tis e h t o t e ta g y lb m e s s A e s U e c n a n e tn ia M ria p e R tn e m e c a lp e R tn e m h s ib ru fe R y g re n e la n o ita re p Oe s u re ta w la n o ita re p Oe s u n o itc u rts n o c -e Dn o itilo m e d tro p s n a rT g n is s e c o rp e ts a W la s o p s iD -e s u e R-y re v o c e R-g n ilc y c e Rla itn e to p
A1 A2 A3 A4 A5 B1 B2 B3 B4 B5 B6 B7 C1 C2 C3 C4 D
X X X MND MND MND MND MNR MNR MNR MND MND X X X X X
RESULTS OF THE LCA - ENVIRONMENTAL IMPACT according to EN 15804+A2: 1 m² Heradesign Corridor Fine (13.3 kg/m²),
Euroclass B
Parameter Unit A1-A3 C1 C2 C3 C4 D
Global Warming Potential total (GWP-total) kg CO 2 eq -9.71E-01 0 4.03E-02 0 7.1E+00 0
Global Warming Potential fossil fuels (GWP-fossil) kg CO 2 eq 5.98E+00 0 4E-02 0 1.98E-01 0
Global Warming Potential biogenic (GWP-biogenic) kg CO 2 eq -6.95E+00 0 0 0 6.95E+00 0
Global Warming Potential luluc (GWP-luluc) kg CO 2 eq 1.67E-03 0 2.69E-04 0 3.66E-04 0
Depletion potential of the stratospheric ozone layer (ODP) kg CFC11 eq 9.17E-12 0 3.92E-15 0 4.66E-13 0
Acidification potential of land and water (AP) mol H+ eq 1.41E-02 0 1.33E-04 0 1.41E-03 0
Eutrophication potential aquatic freshwater (EP-freshwater) kg P eq 1.1E-05 0 1.43E-07 0 3.36E-07 0
Eutrophication potential aquatic marine (EP-marine) kg N eq 4.01E-03 0 6.1E-05 0 3.6E-04 0
Eutrophication potential terrestrial (EP-terrestrial) mol N eq 4.33E-02 0 6.83E-04 0 3.95E-03 0
Formation potential of tropospheric ozone photochemical oxidants kg NMVOC
1.16E-02 0 1.2E-04 0 1.09E-03 0
(POCP) eq
Abiotic depletion potential for non fossil resources (ADPE) kg Sb eq 5.58E-07 0 4.02E-09 0 2.03E-08 0
Abiotic depletion potential for fossil resources (ADPF) MJ 6.94E+01 0 5.24E-01 0 2.6E+00 0
m3 world eq
Water use (WDP) 3.04E-01 0 4.47E-04 0 2.18E-02 0
deprived
RESULTS OF THE LCA - INDICATORS TO DESCRIBE RESOURCE USE according to EN 15804+A2: 1 m² Heradesign Corridor
Fine (13.3 kg/m²), Euroclass B
Parameter Unit A1-A3 C1 C2 C3 C4 D
Renewable primary energy as energy carrier (PERE) MJ 2E+01 0 3.63E-02 0 3.9E-01 0
Renewable primary energy resources as material utilization
MJ 6.98E+01 0 0 0 0 0
(PERM)
Total use of renewable primary energy resources (PERT) MJ 8.98E+01 0 3.63E-02 0 3.9E-01 0
Non renewable primary energy as energy carrier (PENRE) MJ 6.94E+01 0 5.26E-01 0 2.6E+00 0
Non renewable primary energy as material utilization (PENRM) MJ 0 0 0 0 0 0
Total use of non renewable primary energy resources (PENRT) MJ 6.94E+01 0 5.26E-01 0 2.6E+00 0
Use of secondary material (SM) kg 3.35E+00 0 0 0 0 0
Use of renewable secondary fuels (RSF) MJ 0 0 0 0 0 0
Use of non renewable secondary fuels (NRSF) MJ 0 0 0 0 0 0
Use of net fresh water (FW) m3 2.33E-02 0 4.2E-05 0 6.6E-04 0
RESULTS OF THE LCA – WASTE CATEGORIES AND OUTPUT FLOWS according to EN 15804+A2:
1 m² Heradesign Corridor Fine (13.3 kg/m²), Euroclass B
Parameter Unit A1-A3 C1 C2 C3 C4 D
Hazardous waste disposed (HWD) kg 3.69E-08 0 2.78E-12 0 1.34E-10 0
Non hazardous waste disposed (NHWD) kg 4.94E-01 0 8.57E-05 0 1.33E+01 0
Radioactive waste disposed (RWD) kg 1.17E-03 0 9.77E-07 0 2.89E-05 0
Components for re-use (CRU) kg 0 0 0 0 0 0
Materials for recycling (MFR) kg 0 0 0 0 0 0
Materials for energy recovery (MER) kg 0 0 0 0 0 0
Exported electrical energy (EEE) MJ 0 0 0 0 0 0
Exported thermal energy (EET) MJ 0 0 0 0 0 0
RESULTS OF THE LCA – additional impact categories according to EN 15804+A2-optional:
1 m² Heradesign Corridor Fine (13.3 kg/m²), Euroclass B
Parameter Unit A1-A3 C1 C2 C3 C4 D
6 Environmental Product Declaration - Knauf Ceiling Solutions GmbH & Co. KG - Heradesign Corridor Fine
Disease
Incidence of disease due to PM emissions (PM) ND ND ND ND ND ND
incidence
Human exposure efficiency relative to U235 (IR) kBq U235 eq ND ND ND ND ND ND
Comparative toxic unit for ecosystems (ETP-fw) CTUe ND ND ND ND ND ND
Comparative toxic unit for humans (carcinogenic) (HTP-c) CTUh ND ND ND ND ND ND
Comparative toxic unit for humans (noncarcinogenic) (HTP-nc) CTUh ND ND ND ND ND ND
Soil quality index (SQP) SQP ND ND ND ND ND ND
The additional and optional impact categories according to EN 15804+A2 are not declared, as the uncertainty of these indicators is to
be classified as high.
Disclaimer – for the indicators 'abiotic depletion potential for non-fossil resources', 'abiotic depletion potential for fossil resources',
'water (user) deprivation potential, deprivation-weighted water consumption':
The results of this environmental impact indicator shall be used with care as the uncertainties on these results are high as there is
limited experience with the indicator.
6. LCA: Interpretation
The following interpretation contains a summary of the LCA Corridor Fine (Euroclass B).
results referenced to a declared unit of 1 m² Heradesign
A comparison of the individual life-cycle phases results in a as energy provision for the process account for the major
clear dominance of the production phase (modules A1–A3), environmental impacts in this context. The chosen background
with the exception of global warming potential (GWP). The data refers to a realistic representation of the upstream
amount of wood stored in the product refers to a negative processes as far as possible.
contribution to global warming potential. This is due to the
sequestration of biogenic carbon of wood during tree growth. What's more, energy provision for the production at
The sequestered carbon does not contribute to global warming Ferndorf represents another important factor in the
as long as it is stored in the biomass. In the case of landfilling, environmental profile of Heradesign ceiling panels.
this carbon content is stored in the product. If the material is
used as secondary material after deconstruction, the stored In contrast to the previous EPD, the replacement of 50 % of the
carbon is emitted during recalcination. caustic calcined magnesite with Knauf secondary causter is
The environmental effects in the production phase are mainly taken into account. This results in further reduction potential
dominated by the upstream production of caustic calcined compared to the various previous EPDs. For example, the
magnesium oxide in the supply chain of Knauf Ceiling potential fossil greenhouse gas emissions are reduced by
Solutions. Direct emissions from the calcination process as well further 17 % (comparison in accordance with EN 15804+A1).
7 Environmental Product Declaration - Knauf Ceiling Solutions GmbH & Co. KG - Heradesign Corridor Fine
7. Requisite evidence
Heradesign acoustic panels are certified with the German schema, the Belgian regulations, the
ecolabel "Blue Angel" (RAL-UZ 132) as well as the Danish Indoor Air Comfort Gold Standard, the BLUE ANGEL, BREEAM
product quality seal for indoor climate (certificate Nr. 056) as NOR and LEED v4
certificate for the environmental friendliness of the products.
AgBB result overview (28 days)
7.1 Testing pretreatment of substances used
No waste wood is used for the production of Heradesign
acoustic panels.
7.2 Leaching
Not applicable. Heradesign products are designed for indoor
use, a leaching measurement is not useful.
7.3 VOC-emissions
Testing authority: Eurofins Product Testing A/S
Test report: VOC Emissionsprüfbericht Indoor Air Comfort
GOLD (07.12.2022)
Number: 392-2022-00379403_A_EN
Test period: 02.11.–30.11.2022
Result: According to the test report, the product fulfils the
requirements of the French VOC-Ordinance, the AgBB
(Committee for health-related evaluation of building products)
8. References
Standards ISO 14025
DIN EN ISO 14025:2011-10, Environmental labels and
DIN 4108-4 declarations - Type III environmental declarations - Principles
DIN 4108-4:2017-03, Thermal insulation and energy economy and procedures.
in buildings - Part 4: Hygrothermal design values.
ISO 14044
EN 1602 ISO 14044:2006-07, Environmental management - Life cycle
DIN EN 1602:2013-05, Thermal insulating products for building assessment - Requirements and guidelines.
applications - Determination of the apparent density.
ISO 50001
EN 12667 EN ISO 50001:2018, Energy mamagement systems -
DIN EN 12667:2001-05, Thermal performance of building Requirements with guidance for use.
materials and products - Determination of thermal resistance by
means of guarded hot plate and heat flow meter methods - ISO 45001
Products of high and medium thermal resistance. DIN EN ISO 45001:2018, Occupational health and safety
management systems – Requirements with guidance for use.
EN 13168
EN 13168:2012+A1:2015, Thermal insulation products for
buildings - Factory made wood wool (WW) products - Further literature
Specification.
AgBB
EN 13501-1 The Committee for Health-related Assessment of Building
EN 13501-1:2007+A1:2009, Fire classification of construction Products (AgBB) developed test criteria and assessment
products and building elements. standards for a uniform and comprehensible health assessment
of building product emissions in Germany.
EN 13964
EN 13964:2014-04-15, Suspended ceilings - Requirements and EAK-code EAK-Code 17 01 07: European Waste Catalogue:
test methods. Mixtures of concrete, brick, tiles and ceramics with the
exception of materials under17 01 06.
EN 15804
DIN EN 15804:2012+A2 2019+AC:2021, Sustainability of ECHA Candidate List
construction works - Environmental Product Declarations - Core Candidate List of substances of very high concern for
rules for the product category of construction products. Authorisation (ECHA Candidate List), retrieved June 27.2024,
published in accordance with Article 59(10) of the REACH
ISO 9001 Regulation. Helsinki: European Chemicals Agency.
EN ISO 9001:2015, Quality management systems -
Requirements. GaBi
GaBi 10, Software-System and Database for Life Cycle
ISO 14001 Engineering. DB 2022.2. Sphera, 1992–2022. Available at:
EN ISO 14001:2015, Environmental management systems - http://documentation.gabisoftware.com
Requirements with guidance for use.
IBU 2021
8 Environmental Product Declaration - Knauf Ceiling Solutions GmbH & Co. KG - Heradesign Corridor Fine
Institut Bauen und Umwelt e.V.: General Programme e.V. (Hrsg.), 2022.
Instructions for the Preparation of EPDs at the Institut Bauen
und Umwelt e.V.. Version 2.0, Berlin: Institut Bauen und Umwelt PCR: Wood cement - Mineral-bonded wooden composites
e.V., 2021. Product category rules for building-related products and
www.ibu-epd.com services. Teil B: Requirements on the EPD for Wood cement -
Mineral-bonded wooden composites, Version v10. Berlin:
PCR part A Institut Bauen und Umwelt e.V. (Hrsg.), 2024.
Product category rules for building-related products and
services. Part: Calculation rules for the life cycle assessment
and requirements on the project report acording EN
15804+A2:2019. Version 1.3. Berlin: Institut Bauen und Umwelt
9 Environmental Product Declaration - Knauf Ceiling Solutions GmbH & Co. KG - Heradesign Corridor Fine
Publisher
Institut Bauen und Umwelt e.V. +49 (0)30 3087748- 0
Hegelplatz 1 info@ibu-epd.com
10117 Berlin www.ibu-epd.com
Germany
Programme holder
Institut Bauen und Umwelt e.V. +49 (0)30 3087748- 0
Hegelplatz 1 info@ibu-epd.com
10117 Berlin www.ibu-epd.com
Germany
Author of the Life Cycle Assessment
Daxner & Merl GmbH +43 676 849477826
Schleifmühlgasse 13/24 office@daxner-merl.com
1040 Wien www.daxner-merl.com
Austria
Owner of the Declaration
Knauf Ceiling Solutions GmbH & Co. KG 0049 8552 422 0
Elsenthal 15 ceiling.solutions@knauf.com
94481 Grafenau www.knaufceilingsolutions.com
Germany
10 Environmental Product Declaration - Knauf Ceiling Solutions GmbH & Co. KG - Heradesign Corridor Fine
