ENVIRONMENTAL PRODUCT DECLARATION
as per ISO 14025 and EN 15804+A2
Owner of the Declaration Rubner Holding AG - S.p.A.
Publisher Institut Bauen und Umwelt e.V. (IBU)
Programme holder Institut Bauen und Umwelt e.V. (IBU)
Declaration number EPD-RUB-20230230-IBC1-EN
Issue date 27.06.2023
Valid to 26.06.2028
Glued laminated timber
Rubner Holding AG - S.p.A
www.ibu-epd.com | https://epd-online.com
1. General Information
Rubner Holding AG - S.p.A Glued laminated timber
Programme holder Owner of the declaration
IBU – Institut Bauen und Umwelt e.V. Rubner Holding AG - S.p.A.
Hegelplatz 1 Handwerkerzone 2
10117 Berlin 39030 Kiens
Germany Italy
Declaration number Declared product / declared unit
EPD-RUB-20230230-IBC1-EN 1 m³ of glued laminated timber [glulam] with an average density of
464 kg/m³
This declaration is based on the product category rules: Scope:
Solid wood products, 01.08.2021 This EPD is based on a declared unit of 1 m³ of glued laminated timber
(PCR checked and approved by the SVR) (moisture of 10 % at a raw density of 464 kg/m³). The results refer to a
representative average of RUBNER glued laminated timber including
standard beams as well as sophisticated 3D-beam components.
Issue date The LCA covers 100 % of the RUBNER group's production referring to its
sites located at Rohrbach (Austria), Ober-Grafendorf (Austria) and Brixen
27.06.2023
(Italy).
The owner of the declaration shall be liable for the underlying information
Valid to
and evidence; the IBU shall not be liable with respect to manufacturer
26.06.2028 information, life cycle assessment data and evidences.
The EPD was created according to the specifications of EN 15804+A2. In
the following, the standard will be simplified as EN 15804.
Verification
The standard EN 15804 serves as the core PCR
Independent verification of the declaration and data according to ISO
14025:2011
internally X externally
Dipl.-Ing. Hans Peters
(Chairman of Institut Bauen und Umwelt e.V.)
Florian Pronold Matthias Schulz,
(Managing Director Institut Bauen und Umwelt e.V.) (Independent verifier)
1 Environmental Product Declaration - Rubner Holding AG - S.p.A - Glued laminated timber
2. Product
Constructional data
2.1 Product description/Product definition
RUBNER glued laminated timber and glued solid timber Name Value Unit
(RUBNER glulam) is a homogenized unidirectional wood-based Wood types by trade names acc. spruce, pine, larch,
-
material that is used in engineered structural timber to EN 1912 Douglas fir
constructions. RUBNER glulam consists of at least two Wood moisture acc. to EN 14080 < 15 %
boards/laminations made from kiln dried coniferous wood
Use of wood preservatives (the Where other
according to EN 1912 which are glued together at their wide
wood preservative test mark to preservative means -
faces. Due to the multi-layer cross-sectional structure combined
DIN 68800-3 must be indicated) are insufficient
with the technically supported strength and stiffness
Bending strength acc. to EN
classification of the raw materials, RUBNER glulam is 24 N/mm²
14080
characterized by a high product quality. As a result of the
industrial manufacturing process, RUBNER glulam exhibits Compressive strength parallel 24 N/mm2
steady mechanical characteristics. In addition to straight acc. to EN 14080
standard beams, RUBNER glulam also includes architecturally Compressive strength
2.5 N/mm2
sophisticated 3D-beam components which are curved arbitrarily rectangular acc. to EN 14080
in space. Rubner glulam has a high dimensional stability and Tensile strength parallel acc. to
19.2 N/mm2
can be characterized as a largely crack-minimized building EN 14080
material. For the placing on the market of the product in the Tensile strength rectangular acc.
European Union/European Free Trade Association (EU/EFTA) to EN 14080 0.5 N/mm2
(with the exception of Switzerland) Regulation (EU) No.
Modulus of elasticity acc. to EN
305/2011/PCR applies. The product needs a Declaration of 11500 N/mm2
14080
Performance taking into consideration hEN 14080 and the CE-
marking. For use, the respective national provisions apply. Shear strength acc. to EN 14080 3.5 N/mm2
Shear modulus acc. to EN 14080 650 N/mm2
2.2 Application
depending on
RUBNER glulam is mainly used as a structural component for Dimensional deviation acc. to EN
geometrical mm
buildings and bridges. 14080
dimensions
2.3 Technical Data Length < 55 m
The performance data of the product are in accordance with the Width (min. - max.) 0.06 to 0.3 m
Declaration of Performance with respect to its essential Height (min. - max.) 0.012 to 4 m
characteristics according to hEN 14080. Gross density acc. to EN 14080 445 kg/m3
RUBNER glulam is produced in accordance with hEN 14080
Surface quality (Possible
with different strength classes. For the strength class GL 24h
characteristic features must be n.r. -
the following applies:
indicated)
Risk class acc. to DIN 68800-3 4 -
Thermal conductivity acc. to EN
0.12 W/(mK)
12664
Specific heat capacity acc. to EN
1.6 kJ/kgK
12664
Calculation value for thermal
n.r. W/(mK)
conductivity
Water vapor diffusion equivalent
air layer thickness acc. to ISO n.r. m
12572
Water vapour diffusion resistance
20 - 50 -
factor acc. to ISO 12572
Formaldehyde emissions acc. to
< E1 μg/m3
EN 14080
RUBNER glulam is manufactured in accordance with hEN
14080 from coniferous species, with priority being given to
spruce, fir, pine, larch or Douglas fir. Other coniferous species
are permissible but not typical.
RUBNER glulam is produced from kiln-dried coniferous wood
with an average wood moisture content of around 10 % to 11 %
at delivery. For bonding, only approved modern low-emission
adhesives according to chapter 2.5 are used.
The mechanical characteristics of RUBNER glulam are in
accordance with strength classes specified in hEN 14080. For
determination of the technical specifications, the declarations of
performance (DOP) in the currently valid versions apply. The
dimensional tolerances are defined in accordance with hEN
14080 and Glued Laminated Timber Data Sheet.
RUBNER glulam is also produced in the form of wide cross-
2 Environmental Product Declaration - Rubner Holding AG - S.p.A - Glued laminated timber
sections with brick-bonded assembling of the single layers. the blanks are planed. If necessary, these single components
The products are manufactured in domestic visual quality, are bonded together to composite beams with oversized final
visual quality or industrial quality according to Glued Laminated cross-section geometry. If necessary the blanks are cut to their
Timber Data Sheet. final complex shapes. To ensure the product quality, a
Use of preventive chemical wood preservatives in accordance treatment with weathering or wood preservatives may be
with DIN 68800-3 is unusual and permitted only if other required for transport to the construction site, storage, and
preservative measures given in DIN 68800-2 are not sufficient during assembly.
on their own.
2.7 Environment and health during manufacturing
2.4 Delivery status During production, there are no negative impacts on water and
RUBNER glulam is produced with the dimensions according to soil. The resulting process wastewater is fed into the local
chapter 2.3 and is delivered in accordance with Glued sewage system and cleaned according to legal regulations. The
Laminated Timber Data Sheet in domestic visual quality, visual resulting exhaust air is cleaned according to the legal
quality or industrial quality. The tolerances according to EN regulations.
14080 are met. Noise emissions from industrial plants are reduced by structural
measures and comply with the legal requirements.
2.5 Base materials/Ancillary materials The manufacturing process applies to all production facilities
RUBNER glulam comprises at least two unidirectional bonded covered by this EPD.
kiln-dried coniferous boards/laminations according to hEN Two thirds of the production volume are produced in facilities
14081. with an environmental management system ISO 14001 and a
quality management system ISO 9001 in place.
The following types of adhesive systems are used for bonding A third of the production volume is produced in facilities with an
the individual components (finger jointing and surface bonding): occupational health and safety management system OHSAS
• Melamine-urea-formaldehyde adhesives (MUF) 18001.
• Melamine adhesives The employee protection in the manufacturing process
• Emulsion polymer isocyanate (EPI) complies with the respective country-specific requirements,
employees are provided with personal protective equipment.
RUBNER glulam contains the following proportions of
2.8 Product processing/Installation
ingredients per m³ on average:
RUBNER glulam can be processed with commercially available
• Coniferous wood (atro), mainly spruce approx. 88-90 % tools. The instructions for occupational safety/assembly are to
• Water approx. 9-10 % be observed.
• Adhesive about 1 - 2.5 %, The proportions of the
adhesives used are based on: About 40 % MUF, 20 % 2.9 Packaging
melamine and about 40 % EPI. Polyethylene foils and polyproplyene film are used in small
In addition, about 85 g/m² of water-based wood stain are quantities during transportation.
applied. This corresponds to about 0.1 % of the product weight.
2.10 Condition of use
The product has an average density of 464 kg/m³. The composition of RUBNER glulam corresponds to the
composition according to Section 2.5 for the entire period of
This product/article/at least one partial article contains use.
substances listed in the candidate list (date: 17.01.2023)
exceeding 0.1 percentage by mass: no. 2.11 Environment and health during use
Environmental protection: According to current knowledge, the
This product/article/at least one partial article contains other intended use of RUBNER glulam does not present any hazards
carcinogenic, mutagenic, reprotoxic (CMR) substances in or impairments to water, air and soil.
categories 1A or 1B which are not on the candidate list, Health protection: Under normal conditions of use, RUBNER
exceeding 0.1 percentage by mass: no. glulam is not expected to cause any damage or impairments to
health.
Biocide products were added to this construction product or it RUBNER glulam subsequently releases formaldehyde during
has been treated with biocide products (this then concerns a life cycle.
treated product as defined by the (EU) Ordinance on Biocide RUBNER glulam bonded with PU and EPI based adhesives
Products No. 528/2012): no. has formaldehyde emission values in the range of the untreated
raw material wood (sawn timber, by 0.004 ml/m³, Meyer, 1994).
2.6 Manufacture RUBNER glulam bonded with MUF or PRF based adhesives
RUBNER glulam is manufactured from sustainable sawn timber has low emissions of formaldehyde, due to the low level of
(PEFC, FSC) sourcing from sustainable forestry. Wet sawn adhesive in its internal structure and due to its particular use.
timber is kiln dried to a moisture content of about 10 % and Measured against the limit value of 0.1 ml/m³ (0.124 mg/m³) of
subsequently pre-planed. To ensure the characteristic values of the Reach Regulation 1907/2006/EG, the measured values in
the RUBNER glulam, all individual boards are visually- or accordance with EN 717-1 can be classified as low. Rubner
machine-graded regarding strength and stiffness. Weak parts of glulam with melamine-based adhesive systems (MUF, PRF)
planks, which reduce the strength and stiffness properties due gives an average emission in the range of 0.01 to 0.02 mg/m³
to the natural growth characteristics of wood, are cut out (Prüfbericht PB/2117078/CT/2021/4/A1). In individual cases,
depending on the grading class. The graded boards are they can amount to about 0.04 mg/m³.
subsequently bonded by finger jointing to endless laminations.
These laminations with infinite length and a thickness up to 90 2.12 Reference service life
mm are subsequently planed and cut to the required length for Glulam has been used in structural timber construction for more
further production. After applying the adhesive to the wide faces than 100 years. When used as designated, no end of durability
of boards/laminations, RUBNER glulam is pressed in a straight must be expected due to its natural durability (protection
or curved press to at least 2-layer glulam blanks. After curing against moisture). When used as designated, the lifetime of
RUBNER glulam is equal to the duration of use of the building.
3 Environmental Product Declaration - Rubner Holding AG - S.p.A - Glued laminated timber
2.13 Extraordinary effects 2.14 Re-use phase
Fire In the event of selective de-construction, RUBNER glulam can
RUBNER glulam is classified in accordance with 2005/610/EC easily be re-used after the end of the structures service life.
and hEN 14080 as follows: The preferred use of RUBNER glulam is in the form of reuse
based on the applicable country-specific requirements.
Fire protection
If it is not re-used, it will be subjected to thermal utilization for
Name Value
the production of heat and electricity due to the high calorific
Building material class D value of approx. 16.5 MJ/kg (at a humidity of u = 12 %) in
Burning droplets d0 compliance with the applicable country-specific requirements.
Smoke gas development s2
2.15 Disposal
If the residues are not used for any other cascading use, waste
Water wood is disposed according to the applicable country-specific
No ingredients are washed out which could be hazardous to requirements. Disposal represents a possible but unusual case.
water. RUBNER glulam is assigned to waste code 17 02 01 in the
European list of waste 2014/955/EU. (Treated glued laminated
Mechanical destruction timber is assigned to waste code 17 02 04).
The fracture behavior of RUBNER glulam is appearance typical
for solid wood. 2.16 Further information
More detailed information is available at: www.rubner.com
3. LCA: Calculation rules
materials (lamellae, adhesive system, etc.) and the
3.1 Declared Unit corresponding transports to the RUBNER production sites
This EPD refers to a declared unit of 1 m³ of glued laminated (Rohrbach, Ober-Grafendorf and Brixen). As the production site
timber produced by the RUBNER group. The declared unit in Rohrbach delivers lamellae to the other RUBNER sites,
refers to an average density of 464 kg/m³ and a wood moisture resulting environmental impacts refer to RUBNER's specific
at delivery of 10 %. production process including drying. Direct emissions from
Declared unit drying are based on worst-case approximations and are
included in the study. Upstream emissions from the use of
Name Value Unit
adhesive systems rely on supplier-specific data.
Declared unit 1 m3 RUBNER produces thermal energy in its own biomass boilers
Gross density 464 kg/m3 at the Rohrbach and Ober-Grafendorf sites, Brixen uses district
Wood moisture at delivery 10 % heating from the municipal utilities. The Austrian sites are
supplied with 100 % green electricity, Brixen is supplied with
The analysed products represent an average of RUBNER
electricity from the Italian grid. Additionally all sites are provided
glued laminated timber produced at the sites Rohrbach (AT),
by their own photovoltaic systems.
Brixen (IT) and Ober-Grafendorf (AT). It includes straight
standard beams as well as 3D-beam components which are
Module C1 | Deconstruction and demolition
curved arbitrarily in space. As production amounts of both
After the removal of building components overlying the product,
variants are balanced within the RUBNER group, the analysed
the joints can simply be loosened by screwing or sawing and
average is considered a realistic representation.
lifted by cranes to the place of removal. Required energy
demand can be neglected. The actual energy demand depends
The declared unit was calculated on a volume-weighted basis.
on the installation of the products and can therefore vary
This EPD refers to an average product manufactured at several
greatly in the building context.
sites. All products undergo the same processing steps. A
possible variability is only expected due to the use of different
Module C2 | Transport to disposal
wood species. The upstream chain for spruce is considered
Module C2 includes the transport to waste treatment. In this
representative. The robustness of the declared LCA values can
case, transport by truck over a transport distance of 50 km is
thus be classified as high.
assumed.
Brixen and Ober-Grafendorf do not only produce glued
Module C3 | Waste processing
laminated timber but also cross laminated and solid structural
In Module C3, the chipping after the removal of the products is
timber, respectively. The allocation of product-specific material
considered. The wooden products and with them the material-
and energy flows is based on physical relationships when
inherent properties leave the product system as secondary
possible. Where necessary, the allocation is based on the
combustibles in module C3.
production volumes of each product line manufactured at the
referring site.
Module C4 | Disposal
The applied scenario declares the energetic recovery of the
3.2 System boundary
wooden products, therefore no environmental impacts are to be
The life cycle assessment of average glued laminated timber
expected from waste processing of the products in C4.
produced by RUBNER refers to a cradle-to-gate analysis of the
environmental impacts with modules C1–C4 and module D
Module D | Benefits and loads beyond the system
(A1–A3 + C + D). The following life cycle phases are part of the
boundary
analysis:
Applying an European average scenario, module D describes
the energetic recovery of the product at the end of life including
Module A1–A3 | Production stage
the corresponding energy substitution potentials.
The production stage includes upstream burdens of raw
4 Environmental Product Declaration - Rubner Holding AG - S.p.A - Glued laminated timber
3.3 Estimates and assumptions 3.6 Data quality
All assumptions are verified through detailed documentation Data collection is based on product-specific questionnaires. It
and correspond to the best possible representation of reality follows an iterative process of clarifying questions via e-mail,
based on the available data. Background data for wood logs telephone calls or in personal/web meetings. Intensive
refer to generic data for spruce logs in bark derived from GaBi discussions between the RUBNER group and Daxner & Merl
database. Spruce represents the majority of wood processed at results in an accurate mapping of product-related material and
RUBNER. The used dataset represents an approximation for all energy flows. This leads to a high quality of foreground data
other species. collected. Data collection relies on a consistent process
Regional applicability of the used background data refers to according to ISO 14044.
average data under European or German conditions taken from
the GaBi database. German data were used for the Austrian The representation of the main raw materials used for the
and Italian market whenever European or regionalised average production of glued laminated timber is based on supplier-
data were not available. specific primary data (lamellae, adhesive systems) leading to a
high data quality.
Emissions from wood drying were included in the calculations
according to Rüter & Diederichs 2012. The technological, geographical and time-related
representativeness of the database was kept in mind when
3.4 Cut-off criteria selecting background data. Whenever specific data were
The LCA model covers all available input and output flows, missing, either generic datasets or representative average data
which can be represented based on robust data and from which were used instead. The implemented GaBi background
a significant contribution can be expected. Data gaps are filled datasets refer to the latest versions available and are carefully
with conservative assumptions of average data or generic data chosen.
if available and are documented accordingly. Only data with a
contribution of less than 1 % were cut off. The assessment of the robustness of the average can be found
Thus, no data were neglected, of which a substantial impact is in Section 3.1.
to be expected. All relevant data were collected
comprehensively. Cutoff material and energy flows were 3.7 Period under review
chosen carefully based on their expected quantitative Foreground data were collected in the 2022 production year,
contribution as well as potential environmental impacts. Thus, it and the data are based on the volumes produced on an annual
can be assumed that the sum of all neglected input flows does basis.
not account for more than 5 % of the total material, water and
energy flows. Environmental impacts of machines, plant and 3.8 Geographic Representativeness
infrastructure were not included. Land or region, in which the declared product system is
manufactured, used or handled at the end of the product´s
3.5 Background data lifespan: Europe
This study uses generic background data for the evaluation of
upstream environmental impacts from GaBi database 2022.2
3.9 Allocation
as well as recognised literature such as Rüter & Diederichs
2012. Carbon content and primary energy content of the products
were assessed based on their material inherent properties
A large amount of the lamellae processed for glued laminated according to underlying physical relationships.
timber at group level is delivered of the RUBNER RHI located in
3.10 Comparability
Rohrbach. Thus, the supply chain for lamellae input is based on
Basically, a comparison or an evaluation of EPD data is only
primary data.
possible if all the data sets to be compared were created
according to EN 15804 and the building context, respectively
The analysis of the major amount of adhesives used for glulam
the product-specific characteristics of performance, are taken
production is based on primary data from RUBNER's suppliers.
into account.
Where necessary, this information was complemented with
estimates ensuring the completeness of the component's
The GaBi background database was used to calculate the LCA
representation in the LCA.
(GaBi 10; 2022.2).
4. LCA: Scenarios and additional technical information
Characteristic product properties of biogenic carbon
Installation into the building (A5)
During tree growth, the wood assimilates carbon dioxide and
The end of life of the product packaging is not declared in
stores biogenic carbon. The carbon stored in the product is
module A5.
declared in the following table.
Name Value Unit
Information on describing the biogenic Carbon Content at Packaging (polypropylene) 0.298 kg
factory gate Packaging (polyethylene) 0.148 kg
Name Value Unit
Biogenic carbon content in product 208 kg C The end-of-life scenario used in this LCA study is based on the
following assumptions:
5 Environmental Product Declaration - Rubner Holding AG - S.p.A - Glued laminated timber
The product reaches the end-of-waste status after removal from
End of life (C1-C4)
the building, transport to processing and chipping of the
Name Value Unit
product. For the end of life of the glued laminated timber
Energy recovery 464 kg product, energy recovery as secondary fuel in a biomass power
plant is assumed. As the main sales market for the solid wood
Reuse, recovery and/or recycling potentials (D), relevant
products is concentrated in the European region, plant-specific
scenario information
characteristic values correspond to a European average
Name Value Unit scenario (EU). The scenario considers a reprocessing rate of
Processing rate 100 % 100 % for the solid wood products after removal from the
Efficiency of power plant 68 % building. This assumption has to be adjusted accordingly when
applying the results in the building context. At the end of life of
the product, the equilibrium moisture is comparable to the
moisture content at delivery. This value can vary depending on
the storage of the product before energy recovery.
6 Environmental Product Declaration - Rubner Holding AG - S.p.A - Glued laminated timber
5. LCA: Results
The following table contains the LCA results for a declared unit of 1 m³ of glued laminated timber produced by the RUBNER group
(464 kg/m³).
DESCRIPTION OF THE SYSTEM BOUNDARY (X = INCLUDED IN LCA; ND = MODULE OR INDICATOR NOT DECLARED; MNR =
MODULE NOT RELEVANT)
Benefits and
Construction loads beyond
Product stage Use stage End-of-life stage
process stage the system
boundaries
la ire ta m w a Ry lp p u s tro p s n a rT g n iru tc a fu n a M e h t m o rf tro p s n a rTe tis e h t o t e ta g y lb m e s s A e s U e c n a n e tn ia M ria p e R tn e m e c a lp e R tn e m h s ib ru fe R y g re n e la n o ita re p Oe s u re ta w la n o ita re p Oe s u n o itc u rts n o c -e Dn o itilo m e d tro p s n a rT g n is s e c o rp e ts a W la s o p s iD -e s u e R-y re v o c e R-g n ilc y c e Rla itn e to p
A1 A2 A3 A4 A5 B1 B2 B3 B4 B5 B6 B7 C1 C2 C3 C4 D
X X X MND MND MND MND MNR MNR MNR MND MND X X X X X
RESULTS OF THE LCA - ENVIRONMENTAL IMPACT according to EN 15804+A2: 1 m³ glued laminated timber (464 kg/m³)
Parameter Unit A1-A3 C1 C2 C3 C4 D
Global Warming Potential total (GWP-total) kg CO 2 eq -6.87E+02 0 1.47E+00 7.71E+02 0 -4.16E+02
Global Warming Potential fossil fuels (GWP-fossil) kg CO 2 eq 7.62E+01 0 1.4E+00 3.42E+00 0 -3.85E+02
Global Warming Potential biogenic (GWP-biogenic) kg CO 2 eq -7.63E+02 0 6.09E-02 7.67E+02 0 -3.06E+01
Global Warming Potential luluc (GWP-luluc) kg CO 2 eq 2.56E-01 0 9.39E-03 7.24E-04 0 -4.61E-02
Depletion potential of the stratospheric ozone layer (ODP) kg CFC11 eq 2.57E-09 0 1.37E-13 5.01E-11 0 -2.98E-09
Acidification potential of land and water (AP) mol H+ eq 6.5E-01 0 4.65E-03 7.52E-03 0 3.19E-01
Eutrophication potential aquatic freshwater (EP-freshwater) kg P eq 3.99E-03 0 4.98E-06 9.99E-06 0 -6.02E-04
Eutrophication potential aquatic marine (EP-marine) kg N eq 2.61E-01 0 2.13E-03 1.69E-03 0 6.92E-02
Eutrophication potential terrestrial (EP-terrestrial) mol N eq 2.3E+00 0 2.38E-02 1.77E-02 0 8.2E-01
Formation potential of tropospheric ozone photochemical oxidants kg NMVOC
7.77E-01 0 4.18E-03 4.56E-03 0 2.94E-01
(POCP) eq
Abiotic depletion potential for non fossil resources (ADPE) kg Sb eq 4.21E-05 0 1.4E-07 9.33E-07 0 -6.4E-05
Abiotic depletion potential for fossil resources (ADPF) MJ 1.05E+03 0 1.83E+01 6.21E+01 0 -6.66E+03
m3 world eq
Water use (WDP) 2.51E+01 0 1.56E-02 7.81E-01 0 -2.19E+01
deprived
RESULTS OF THE LCA - INDICATORS TO DESCRIBE RESOURCE USE according to EN 15804+A2: 1 m³ glued laminated
timber (464 kg/m³)
Parameter Unit A1-A3 C1 C2 C3 C4 D
Renewable primary energy as energy carrier (PERE) MJ 4.08E+03 0 1.27E+00 7.71E+03 0 -2.06E+03
Renewable primary energy resources as material utilization
MJ 7.67E+03 0 0 -7.67E+03 0 0
(PERM)
Total use of renewable primary energy resources (PERT) MJ 1.18E+04 0 1.27E+00 3.45E+01 0 -2.06E+03
Non renewable primary energy as energy carrier (PENRE) MJ 9.06E+02 0 1.84E+01 1.92E+02 0 -6.67E+03
Non renewable primary energy as material utilization (PENRM) MJ 1.49E+02 0 0 -1.3E+02 0 0
Total use of non renewable primary energy resources (PENRT) MJ 1.06E+03 0 1.84E+01 6.22E+01 0 -6.67E+03
Use of secondary material (SM) kg 0 0 0 0 0 0
Use of renewable secondary fuels (RSF) MJ 0 0 0 0 0 7.67E+03
Use of non renewable secondary fuels (NRSF) MJ 0 0 0 0 0 1.3E+02
Use of net fresh water (FW) m3 1.09E+00 0 1.46E-03 3.29E-02 0 -1.4E+00
RESULTS OF THE LCA – WASTE CATEGORIES AND OUTPUT FLOWS according to EN 15804+A2:
1 m³ glued laminated timber (464 kg/m³)
Parameter Unit A1-A3 C1 C2 C3 C4 D
Hazardous waste disposed (HWD) kg 4.27E-07 0 9.71E-11 5.37E-09 0 -8.25E-07
Non hazardous waste disposed (NHWD) kg 3.54E+00 0 2.99E-03 4.68E-02 0 2.31E-01
Radioactive waste disposed (RWD) kg 1.88E-02 0 3.41E-05 9.93E-03 0 -5.9E-01
Components for re-use (CRU) kg 0 0 0 0 0 0
Materials for recycling (MFR) kg 0 0 0 0 0 0
Materials for energy recovery (MER) kg 0 0 0 4.64E+02 0 0
Exported electrical energy (EEE) MJ 0 0 0 0 0 0
Exported thermal energy (EET) MJ 0 0 0 0 0 0
RESULTS OF THE LCA – additional impact categories according to EN 15804+A2-optional:
1 m³ glued laminated timber (464 kg/m³)
Parameter Unit A1-A3 C1 C2 C3 C4 D
Incidence of disease due to PM emissions (PM) Disease ND ND ND ND ND ND
7 Environmental Product Declaration - Rubner Holding AG - S.p.A - Glued laminated timber
incidence
Human exposure efficiency relative to U235 (IR) kBq U235 eq ND ND ND ND ND ND
Comparative toxic unit for ecosystems (ETP-fw) CTUe ND ND ND ND ND ND
Comparative toxic unit for humans (carcinogenic) (HTP-c) CTUh ND ND ND ND ND ND
Comparative toxic unit for humans (noncarcinogenic) (HTP-nc) CTUh ND ND ND ND ND ND
Soil quality index (SQP) SQP ND ND ND ND ND ND
The additional and optional impact categories according to EN 15804+A2 are not declared, as the uncertainty of these indicators is to
be classified as high.
Disclaimer 1 – for the indicator 'Potential Human exposure efficiency relative to U235'.
This impact category deals mainly with the eventual impact of lowdose ionizing radiation on human health of the nuclear fuel cycle. It
does not consider effects due to possible nuclear accidents, occupational exposure or radioactive waste disposal in underground
facilities. Potential ionizing radiation from the soil, from radon and from some construction materials is also not measured by this
indicator.
Disclaimer 2 – for the indicators 'abiotic depletion potential for non-fossil resources', 'abiotic depletion potential for fossil resources',
'water (user) deprivation potential, deprivation-weighted water consumption', 'potential comparative toxic unit for ecosystems', 'potential
comparative toxic unit for humans – cancerogenic', 'Potential comparative toxic unit for humans - not cancerogenic', 'potential soil
quality index'.
The results of this environmental impact indicator shall be used with care as the uncertainties on these results are high as there is
limited experience with the indicator.
6. LCA: Interpretation
The following interpretation contains a summary of the LCA After its use in the building, the product is assumed to be
results referenced to a declared unit of 1 m³ of glued laminated incinerated in a biomass power plant. As a result, the
timber. incorporated carbon is emitted again to the atmosphere
representing biogenic carbon dioxide emissions (module C3).
The global warming potential (GWP) of glued laminated timber
shows negative values in the production phase (modules A1– The negative values in the end-of-life (module D) result from
A3). These negative impacts results from the use of wood as the energetic treatment of the product. As the energy produced
raw material. Wood sequesters biogenic carbon during tree at the biomass power plant can substitute (mainly fossil) fuels,
growth. The sequestered carbon does not contribute to global an environmental net benefit is generated.
warming as long as it is stored in the biomass.
Potential global warming (GWP) due to the production of carbon neutral, as the wood is derived from sustainably
Rubner glulam mainly stems from the provision of round wood managed forests.
and associated impacts due to forestry. The processing of the
products includes the use of all wooden residues for heat What's more, the electricity demand at the Italian production
production. Its thermal treatment is taken into account as site (mainly fossil fuels in the Italian residual mix) and the
8 Environmental Product Declaration - Rubner Holding AG - S.p.A - Glued laminated timber
production of the ahdesive system represent main drivers of The presented results are considered to be representative for
global warming potential. all RUBNER production sites. It refers to an average product
based on the weighted production volumes of each site.
Due to the use of green electricity in the production sites of
Rohrbach and Ober-Grafendorf, the The results of the previous EPD (EPD-RUB-20180058-IBB1-
external supply of electricity at the sites represents a minor EN) are not directly comparable with the present updated
factor in the environmental profile of the product. version due to the update of the underlying methodology
according to EN 15804+A2.
7. Requisite evidence
The following evidence of environmental and health relevance 7.2 MDI
was provided. When gluing RUBNER glulam with MDI-based adhesive, the
contained MDI will react completely. Thus, a MDI emission from
7.1 Formaldehyde the finished Rubner glulam is not possible. As there is no
The emissions (melamine-based adhesive systems) listed in standardised measurement process defined in test standards,
section 2.11 are based on test results of emission no test reports are available.
measurements in accordance with EN 717-1 at a temperature For the verification of the workplace concentration of MDI (acc.
of 23 °C, a relative humidity of 45 % and an air change rate of to EN 689), a test report is available (date 8.8 2022), the
1.0 per hour. Within the framework of the tests, the adhesives maximum allowed workplace concentration of 0.005 mg/m³ is
were investigated in combination with the types of wood significantly higher than a measurement with <0.0005 mg/m³
species. The test results all meet the requirements of emission has shown.
class E1 according to hEN 14080: 2013 of 0.124 mg/m³.
One test report (No 16F6001, 2016) defines a formaldehyde 7.3 Fire gas toxicity
emission of 0.01 mg/m³ for Rubner glulam with melamine- Due to the heterogeneous structure of glued laminated timber,
based adhesive. combined with the non-applicability of the test standard DIN
One test report (E-CMP / KT T410 405, 2016) defines a 53436, no relevant measurement results are available, the test
formaldehyde emission depending on the wood species with specimen geometry is not able to represent the real gas
0.022 mg/m³ for spruce, 0.037 mg/m³ for pine, 0.010 mg/m³ for composition for a representative cross-section.
larch and 0.007 mg/m³ for Douglas fir for Rubner glulam with
melamine-based adhesive. 7.4 VOC emissions
One test report in accordance with EN 717-1 For the verification of VOC emissions, a test report (51005-001
(2117078/CT/2021/4/A1, 2021) defines a formaldehyde (III), 2016) of an emission analysis according to AgBB-Scheme
emission confirms a formaldehyde emission below the technical 2015 is available. Analysis was performed in accordance with
detection limit. ISO 16000-3 and ISO 16000-6.
Additionally a test report (PB/2117078/CT/1, 2021) of an
There is a test report for proof of occupational exposure emission analysis according to AgBB-Scheme 2018 is
(according to EN 689 (date 31. 3. 2016), the maximum allowed available. Analysis was performed in accordance with DIN EN
workplace concentration of 0.246 mg/m³ is significantly higher 16516.
than two measurements with 0.0075 and 0.086 mg/m³ have
VOC emissions
shown.
Name Value Unit
There is a test report for proof of occupational exposure Overview of Results (28 days) - μg/m3
(according to EN 689 (date 8. 8 2022), the maximum allowed TVOC (C6 - C16) acc. to AgBB 2018 125 μg/m3
workplace concentration of 0.369 mg/m³ is significantly higher
Sum SVOC (C16 - C22) acc. to AgBB 2015 < 5 μg/m3
than the measured with concentration of 0.12 mg/m³ have
R (dimensionless) acc. to AgBB 2018 0,18 -
shown.
For RUBNER glulam glued with EPI adhesives, according to VOC without NIK acc. to AgBB 2015 <5 μg/m3
the manufacturer of the glue, no formaldehyde is added to the Carcinogenic Substances <1 μg/m3
glulam system via the adhesive; the emissions are in the range
of natural wood.
8. References
Standards EN 689
EN 689:1995, Workplace atmospheres - Guidance for the
DIN 53436 assessment of exposure by inhalation to chemical agents for
DIN 53436:2015, Generation of thermal decomposition comparison with limit values and measurement strategy.
products from materials for their analytic-toxicological testing.
EN 717-1
DIN 68800-2 DIN EN 717-1:2005-01, Wood-based panels – Determination of
DIN 68800-2:2012-02, Wood preservation – Part 2: Preventive Formaldehyde release – Part 1: Formaldehyde emission by the
constructional measures in buildings. chamber method.
DIN 68800-3 EN 1912
DIN 68800-3:2012-02, Wood preservation – Part 3: Preventive EN 1912:2013-10-15, Structural timber - Strength classes -
protection of wood with wood preservatives. Assignment of visual grades and species.
9 Environmental Product Declaration - Rubner Holding AG - S.p.A - Glued laminated timber
EN 12664 REACH Regulation. European Chemicals Agency.
EN 12664:2001, Thermal performance of building materials and
products - Determination of thermal resistance by means of GaBi
guarded hot plate and heat flow meter methods - Dry and moist GaBi 10, Software-System and Database for Life Cycle
products with medium and low thermal resistance. Engineering. 2022.2. Stuttgart, Echterdingen: Sphera, 1992-
2022. Available at: https://sphera.com/product-sustainability-
EN 15804 gabi-data-search/
DIN EN 15804:2012+A2:2019+AC:2021, Sustainability of
construction works Environmental product declarations Core Glued Laminated Timber Data Sheet
rules for the product category of construction products. (BS-Holz-Merkblatt), der Studiengemeinschaft Holzleimbau
e.V., 2019 (in German).
hEN 14080
hEN 14080:2013, Timber structures — Glued laminated timber IBU 2021
and glued solid timber — Requirements. Institut Bauen und Umwelt e.V.: General Programme
Instructions for the Preparation of EPDs at the Institut Bauen
hEN 14081 und Umwelt e.V. (IBU). Version 2.0, Berlin: Institut Bauen und
hEN 14081-1:2016-06-01, Timber structures - Strength graded Umwelt e.V., 2021. www.ibuepd.com
structural timberwith rectangular cross section - Part 1: General
requirements. Meyer, 1994
Meyer, B, Boehme, C: 1994, Formaldeyhdabgabe von natürlich
ISO 9001 gewachsenem Holz, Holzzentralblatt 122 (Formaldeyhd release
EN ISO 9001:2015, Qualitätsmanagementsysteme - of naturally grown wood), S 1969-1972.
Anforderungen.
Ordinance on Biocide Products
ISO 12572 Regulation (EU) No 528/2012 of the European Parliament and
EN ISO 12572:2016, Hygrothermal performance of building of the Council of 22 May 2012 concerning the making available
materials and products - Determination of water vapour on the market and use of biocidal products.
transmission properties - Cup method.
PCR part A
ISO 14001 Product category rules for building-related products and
EN ISO 14001:2015, Environmental management systems - services. Part A: Calculation Rules for the Life Cycle
Requirements with guidance for use. Assessment and Requirements on the Project Report according
to EN 15804+A2:2019. Version 1.3. Berlin: Institut Bauen und
ISO 14025 Umwelt e.V., 2022.
DIN EN ISO 14025:2011-10, Environmental labels and
declarations Type III environmental declarations Principles and PCR: Solid wood products
procedures. Product category rules for building-related products and
services. Part B: EPD requirements for solid wood products.
ISO 14044 Version v2, Berlin: Institut Bauen und Umwelt e.V., 31.05.2023.
DIN EN ISO 14044:2006-10, Environmental management - Life
cycle assessment - Requirements and guidelines. PCR 305/2011 (EU)
REGULATION (EU) No 305/2011 OF THE EUROPEAN
ISO 16000-3 PARLIAMENT AND OF THE COUNCIL of 9 March 2011 laying
ISO 16000-3:2011, Indoor air - Part 3: Determination of down harmonised conditions for the marketing of construction
formaldehyde and other carbonyl compounds in indoor air and products and repealing Council Directive 89/106/EEC
test chamber air - Active sampling method.
Rüter & Diederichs 2012
ISO 16000-6 Ökobilanz-Basisdaten für Bauprodukte aus Holz. Work report
ISO 16000-6:2011, Indoor air - Part 6: Determination of volatile from the Institut für Holztechnologie und Holzbiologie Nr.
organic compounds in indoor and test chamber air by active 2012/1. Hamburg: Johann Heinrich von Thünen-Institut.
sampling on Tenax TA® sorbent, thermal desorption and gas
chromatography using MS or MS-FID. 2005/610/EG
2005/610/EG, COMMISSION DECISION of 9 August 2005
OHSAS 18001 establishing the classes of reaction-to-fire performance for
OHSAS 18001:2018, Occupational Health- and Safety certain construction products.
Assessment Series.
2014/955/EU
2014/955/EU,COMMISSION DECISION of 18 December 2014
Further references amending Decision 2000/532/EC on the list of waste pursuant
to Directive 2008/98/EC of the European Parliament and of the
AgBB-Scheme 2015 Council.
German Committee for HealthRelated Evaluation of Building
Products (AgBB): Approach to health assessment of emissions 1907/2006/EG
of volatile organic compounds (VOCs and SVOCs) from VERORDNUNG (EG) Nr. 1907/2006 DES EUROPÄISCHEN
building products. PARLAMENTS UND DES RATES vom 18. Dezember 2006 zur
Registrierung, Bewertung, Zulassung und Beschränkung
Candidate List chemischer Stoffe (REACH).
List of substances of very high concern considered for approval
(status 17.01.2023) according to Article 59 para. 10 of the
10 Environmental Product Declaration - Rubner Holding AG - S.p.A - Glued laminated timber
Publisher
Institut Bauen und Umwelt e.V. +49 (0)30 3087748- 0
Hegelplatz 1 info@ibu-epd.com
10117 Berlin www.ibu-epd.com
Germany
Programme holder
Institut Bauen und Umwelt e.V. +49 (0)30 3087748- 0
Hegelplatz 1 info@ibu-epd.com
10117 Berlin www.ibu-epd.com
Germany
Author of the Life Cycle Assessment
Daxner & Merl GmbH +43 676 849477826
Schleifmühlgasse 13/24 office@daxner-merl.com
1040 Wien www.daxner-merl.com
Austria
Owner of the Declaration
Rubner Holding AG - S.p.A. 0039 0474 563 777
Handwerkerzone 2 info@rubner.com
39030 Kiens www.rubner.com
Italy
11 Environmental Product Declaration - Rubner Holding AG - S.p.A - Glued laminated timber
