ENVIRONMENTAL PRODUCT DECLARATION
as per ISO 14025 and EN 15804+A2
Owner of the Declaration dormakaba International Holding GmbH
Publisher Institut Bauen und Umwelt e.V. (IBU)
Programme holder Institut Bauen und Umwelt e.V. (IBU)
Declaration number EPD-DOR-20220087-CBA3-EN
Issue date 17.03.2022
Valid to 16.03.2027
EntriWorX Unit 92 40
dormakaba
www.ibu-epd.com | https://epd-online.com
General Information
dormakaba EntriWorX Unit 92 40
Programme holder Owner of the declaration
IBU – Institut Bauen und Umwelt e.V. dormakaba International Holding GmbH
Hegelplatz 1 DORMA Platz 1
10117 Berlin 58256 Ennepetal
Germany Germany
Declaration number Declared product / declared unit
EPD-DOR-20220087-CBA3-EN 1 piece of the product: EntriWorX Unit 92 40
This declaration is based on the product category rules: Scope:
Electronic and physical Access Control Systems, 01.08.2021 This EPD refers to a specific product manufactured by dormakaba. The
(PCR checked and approved by the SVR) production site is located in Villingen-Schwenningen (Germany).
The data represents the year 2020.
Issue date The owner of the declaration shall be liable for the underlying information
and evidence; the IBU shall not be liable with respect to manufacturer
17.03.2022
information, life cycle assessment data and evidences.
The EPD was created according to the specifications of EN 15804+A2. In
Valid to
the following, the standard will be simplified as EN 15804.
16.03.2027
Verification
The standard EN 15804 serves as the core PCR
Independent verification of the declaration and data according to ISO
14025:2011
internally X externally
Dipl.-Ing. Hans Peters
(Chairman of Institut Bauen und Umwelt e.V.)
Florian Pronold Dr.-Ing. Wolfram Trinius,
(Managing Director Institut Bauen und Umwelt e.V.) (Independent verifier)
1 Environmental Product Declaration - dormakaba - EntriWorX Unit 92 40
Product
• 1x RS-485
Product description/Product definition • 1x RS-232
The EntriWorX Unit 92 40 is the central control unit for different • 1x CAN Bus
domains like access control, escape route management and • 3x potential-free relays, 30 V AC/DC; max. 2 A
door sequence control. It is capable of managing simple or • 4x digital inputs
even complex entrance and exit door configurations. • 1x tamper contact
Based on a state-of-the-art operating system the EntriWorX
Control Unit is a modern IoT edge device respecting IT security Power supply
requirements and enabling connectivity to cloud services. • PoE, as per IEEE 802.3af
Power supply via PoE and a compact design allows easy • PoE+, as per IEEE 802.3at
integration in SOHO as well as in Enterprise environments.
Standardized interface and protocols based on RS-485 and Output voltage
CAN facilitate the integration of peripheral devices. For the • Reader: 5/12 V DC
placing on the market in the European Union/European Free • Elec. door opener: 12/24 V DC
Trade Association (EU/EFTA) (with the exception of
Switzerland) the following legal provisions apply: Class of protection as per EN 60529:IP40.
• Electromagnetic The product is not harmonised in accordance with the
Compatibility Directive (EMC) Construction Product Regulations (CPR) but in accordance with
• Low Voltage other provisions for harmonisation of the EU. Compliance with
Directive (LVD) the European Union Directive and technical specifications:
• Restriction of • EN 55032:2015
Hazardous Substances (RoHS) • EN 55024:2010 + A1:2015
• Radio Equipment Directive (RED) • EN 50364:2010
• EN 50581:2012 • EN 62368-1:2014 + A11:2017
• EN 60529:2014
The CE-marking takes into account the proof of conformity with • EN 301489-1 V2.2.1 Draft
the respective harmonized standards based on the legal • EN 301489-3 V2.1.1
provisions above. For the application and use the respective • EN 300330 V2.1.1
national
provisions apply. The product is subject to CE marking according to the relevant
harmonization legislation.
Application
In addition, the product also conforms to the following
The EntriWorX Unit 92 40 networks the door technology standards:
components through simple plug & play instead of complex
• UL 294:2013
wiring and different transmission protocols and enables the
• UL62368-1:2014-12
commissioning of door systems based on a simple app. This
• CAN/CSA-22.2
setup app simplifies commissioning based on pre-configured
No. 62368-1:2014-12
parameters and provides all the information needed for
• FCC
installation. Once the building is in operation, the data from the
connected door components can then be transferred to a
Base materials/Ancillary materials
higher-level system for controlling the processes in the building.
The major material
This can be an existing system of the customer or EntriWorX
compositions including packaging of the product are listed
Insights.
below:
Technical Data Name Value Unit
The EntriWorX Unit 92 40 has the following technical Plastics 48,5 %
properties: Paper 27 %
Name Value Unit
Electronics 23,5 %
Operating Temperature 0 - 50 °C
Steel 1 %
Operating Humidity 5 - 85 %
The product includes partial articles which contain substances
Height Dimension 208 mm
listed in the Candidate List of REACH Regulation
Width Dimension 208 mm 1907/2006/EC (date: 17.01.2022) exceeding 0.1 percentage by
Depth Dimension 48 mm mass in the alloy: yes
Weight (without packaging) 0,675 kg • Lead (Pb): 7439-92-1 (CAS No.) is included in some of
Weight (with packaging) 0,923 kg the alloys used. The concentration of lead in each
Power consumption "idle mode" 5 W individual alloy does not exceed 4.0% (by mass).
• Lead titanium trioxide (O3 Pb Ti): 12060-00-03
Power consumption "on mode" 12 W
The Candidate List can be found on the ECHA website
Host Interface address: https:echa.europa.eu/de/home.
• Ethernet 10/100 Mbit/s
Reference service life
Peripherals Interface The reference service life of the dormakaba EntriWorX Unit 92
Variant MRD 40 is estimated to be 15 years. This number is based on the
• 2x coaxial for registration units (LEGIC / MIFARE) support and service life and is not an estimated lifetime.
2 Environmental Product Declaration - dormakaba - EntriWorX Unit 92 40
LCA: Calculation rules
including provision of all materials, products and energy, as well
Declared Unit as waste processing up to the end-of-waste state or disposal of
The declared unit is 1 piece of the product: EntriWorX Unit 92 final residues during the construction process stage.
40.
Name Value Unit Use stage - Module B6
Declared unit 1 pce. The use stage related to the operation of the building includes:
— B6, operational energy use
Conversion factor to 1 kg (kg per declared unit) 1.08 -
Product weight including packaging 0,923 kg
End-of-life stage– Modules C1-C4 and D
The end-of-life stage includes:
System boundary — C1, de-construction, demolition:
The type of EPD is: cradle to gate with options, modules C1– — C2, transport to waste processing;
C4, and module D (A1–A3 + C + D and additional modules: A4 — C3, waste processing for reuse, recovery and/or recycling;
+ A5 + B6) — C4, disposal; including provision and all transport, provision
of all materials, products and related energy and water use.
Production - Module A1-A3
The product stage includes: Module D (Benefits and loads beyond the system boundary)
includes:
— A1, raw material extraction, processing and mechanical — D, recycling potentials, expressed as net impacts and
treatments, processing of benefits.
secondary material input (e.g. recycling processes),
— A2, transport to the manufacturer, Geographic Representativeness
— A3, manufacturing and assembly Land or region, in which the declared product system is
manufactured, used or handled at the end of the product´s
including provision of all materials, products and energy, as well lifespan: Germany
as waste processing up
to the end-of waste state.
Comparability
Construction stage - Modules A4-A5 Basically, a comparison or an evaluation of EPD data is only
The construction process stage includes: possible if all the data sets to be compared were created
— A4, transport to the building site; according to EN 15804 and the building context, respectively
— A5, installation into the building; the product-specific characteristics of performance, are taken
into account. Background database: GaBi, SP40.
LCA: Scenarios and additional technical information
Operational energy use (B6) and Operational water use
Characteristic product properties of biogenic carbon
(B7)
Information on describing the biogenic Carbon Content at The use stage is declared for 15 years.
factory gate
Name Value Unit
Name ValueUnit
Energy consumption for 1 year 54.02 kWh
kg
Biogenic carbon content in product 0.01 on mode per day 4 h
C
idle mode 20 h
Biogenic carbon content in accompanying kg
0.1 on mode power 12 W
packaging C
idle mode 5 W
Days per year in use 365 days
The following technical scenario information is required for the
declared modules.
End of life (C1-C4)
Transport to the building site (A4) C1: The product dismantling from the building is done manually
Name Value Unit without environmental burden.
Litres of fuel per 1 kg (truck) 0.00276 l/100km C2: Transport to waste treatment at end of life is 50km.
Transport distance (truck) 750 km Name Value Unit
Capacity utilisation (including empty runs) 51 % Recycling (Steel) 0.01 kg
Transort distance (ship) 1000 km Energy recovery (Plastic) 0.43 kg
Energy recovery (Paper) 0,02 kg
Installation into the building (A5)
Recycling and landfilling (Electronics) 0,21 kg
Name Value Unit
Transportation to Waste 50 km
Waste Packaging (paper) 0.227 kg
Region for end of life: Global
Waste Packaging (plastic) 0,022 kg
Reuse, recovery and/or recycling potentials (D), relevant
Reference service life
scenario information
Name Value Unit
Collection rate is 100%.
Life Span according to the manufacturer 15 a
3 Environmental Product Declaration - dormakaba - EntriWorX Unit 92 40
LCA: Results
DESCRIPTION OF THE SYSTEM BOUNDARY (X = INCLUDED IN LCA; MND = MODULE OR INDICATOR NOT DECLARED; MNR
= MODULE NOT RELEVANT)
Benefits and
Construction loads beyond
Product stage Use stage End of life stage
process stage the system
boundaries
la ire ta m w a Ry lp p u s tro p s n a rT g n iru tc a fu n a M e h t m o rf tro p s n a rTe tis e h t o t e ta g y lb m e s s A e s U e c n a n e tn ia M ria p e R tn e m e c a lp e R tn e m h s ib ru fe R y g re n e la n o ita re p Oe s u re ta w la n o ita re p Oe s u n o itc u rts n o c -e Dn o itilo m e d tro p s n a rT g n is s e c o rp e ts a W la s o p s iD -e s u e R-y re v o c e R-g n ilc y c e Rla itn e to p
A1 A2 A3 A4 A5 B1 B2 B3 B4 B5 B6 B7 C1 C2 C3 C4 D
X X X X X MND MND MNR MNR MNR X MND MND X X X X
RESULTS OF THE LCA - ENVIRONMENTAL IMPACT according to EN 15804+A2: 1 piece EntriWorX Unit 92 40
Parameter Unit A1-A3 A4 A5 B6 C2 C3 C4 D
GWP-total kg CO 2 eq 1.59E+01 6.36E-02 3.75E-01 4.13E+02 2.98E-03 1.08E+00 4.05E-04 -1.24E+00
GWP-fossil kg CO 2 eq 1.61E+01 6.09E-02 6.16E-02 4.11E+02 2.85E-03 1.08E+00 4.02E-04 -1.24E+00
GWP-biogenic kg CO 2 eq -2.4E-01 2.68E-03 3.14E-01 8.16E-01 1.32E-04 2.53E-05 1.37E-06 1.69E-04
GWP-luluc kg CO 2 eq 2.31E-02 1.44E-06 8.32E-06 5.78E-01 6.78E-08 6.13E-05 1.16E-06 -1.45E-03
ODP kg CFC11 eq 1.75E-09 6.39E-18 8.5E-17 6.2E-12 3.01E-19 5.47E-16 1.49E-18 -8.26E-15
AP mol H+ eq 8.57E-02 1.69E-04 9.97E-05 1.83E+00 2.85E-06 1.93E-04 2.88E-06 -1.14E-02
EP-freshwater kg P eq 1.14E-04 1.31E-08 1.56E-08 7.83E-04 6.1E-10 8.73E-08 6.9E-10 -1.18E-06
EP-marine kg N eq 1.52E-02 4.78E-05 3.47E-05 3E-01 9.07E-07 4.35E-05 7.42E-07 -9.75E-04
EP-terrestrial mol N eq 1.62E-01 5.26E-04 4.49E-04 3.23E+00 1.01E-05 8.8E-04 8.16E-06 -1.05E-02
kg NMVOC
POCP 4.47E-02 1.34E-04 9.22E-05 8.67E-01 2.56E-06 1.21E-04 2.25E-06 -3.19E-03
eq
ADPE kg Sb eq 1.31E-01 1.81E-09 1.29E-09 8.48E-05 8.54E-11 7.5E-09 3.61E-11 -4.92E-04
ADPF MJ 2.07E+02 8.57E-01 1.26E-01 6.19E+03 4.04E-02 5.03E-01 5.27E-03 -1.79E+01
m3 world eq
WDP 3.51E+00 1.19E-04 4.54E-02 8.74E+01 5.58E-06 1.11E-01 4.21E-05 -3.54E-01
deprived
GWP = Global warming potential; ODP = Depletion potential of the stratospheric ozone layer; AP = Acidification potential of land and water; EP =
Eutrophication potential; POCP = Formation potential of tropospheric ozone photochemical oxidants; ADPE = Abiotic depletion potential for non-fossil
resources; ADPF = Abiotic depletion potential for fossil resources; WDP = Water (user) deprivation potential)
RESULTS OF THE LCA - INDICATORS TO DESCRIBE RESOURCE USE according to EN 15804+A2: 1 piece EntriWorX Unit 92
40
Parameter Unit A1-A3 A4 A5 B6 C2 C3 C4 D
PERE MJ 4.5E+01 2.71E-03 2.75E+00 2.32E+03 1.27E-04 3.95E-01 6.91E-04 -3.05E+00
PERM MJ 4.8E+01 0 -2.72E+00 0 0 -2.64E-01 0 0
PERT MJ 2.36E+02 2.71E-03 2.49E-02 2.32E+03 1.27E-04 1.31E-01 6.91E-04 -3.05E+00
PENRE MJ 2.07E+02 8.58E-01 1.03E+00 6.2E+03 4.04E-02 1.59E+01 5.28E-03 -1.79E+01
PENRM MJ 2.24E+02 0 -9.05E-01 0 0 -1.54E+01 0 0
PENRT MJ 2.08E+02 8.58E-01 1.26E-01 6.2E+03 4.04E-02 5.03E-01 5.28E-03 -1.79E+01
SM kg 7.1E-03 0 0 0 0 0 0 0
RSF MJ 0 0 0 0 0 0 0 0
NRSF MJ 9.51E-02 0 0 0 0 0 0 0
FW m3 9.51E-02 4.86E-06 1.07E-03 3.16E+00 2.28E-07 2.65E-03 1.33E-06 -7.79E-03
PERE = Use of renewable primary energy excluding renewable primary energy resources used as raw materials; PERM = Use of renewable primary
energy resources used as raw materials; PERT = Total use of renewable primary energy resources; PENRE = Use of non-renewable primary energy
excluding non-renewable primary energy resources used as raw materials; PENRM = Use of non-renewable primary energy resources used as raw
materials; PENRT = Total use of non-renewable primary energy resources; SM = Use of secondary material; RSF = Use of renewable secondary fuels;
NRSF = Use of non-renewable secondary fuels; FW = Use of net fresh water
RESULTS OF THE LCA – WASTE CATEGORIES AND OUTPUT FLOWS according to EN 15804+A2:
1 piece EntriWorX Unit 92 40
Parameter Unit A1-A3 A4 A5 B6 C2 C3 C4 D
HWD kg 1.39E-05 8.33E-11 2.44E-10 2.87E-06 3.92E-12 1.92E-09 8.04E-11 -3.1E-08
NHWD kg 5.21E-01 8.77E-05 1.56E-02 3.87E+00 4.13E-06 1.13E-01 2.65E-02 -1.4E-01
RWD kg 4.8E-03 9.22E-07 6.26E-06 7.18E-01 4.34E-08 1.87E-05 6E-08 -7.74E-04
CRU kg 0 0 0 0 0 0 0 0
MFR kg 0 0 0 0 0 2.28E-01 0 0
MER kg 0 0 0 0 0 0 0 0
EEE MJ 1.07E-01 0 5.86E-01 0 0 0 0 0
EET MJ 1.95E-01 0 1.11E+00 0 0 0 0 0
4 Environmental Product Declaration - dormakaba - EntriWorX Unit 92 40
HWD = Hazardous waste disposed; NHWD = Non-hazardous waste disposed; RWD = Radioactive waste disposed; CRU = Components for re-use;
MFR = Materials for recycling; MER = Materials for energy recovery; EEE = Exported electrical energy; EET = Exported thermal energy
RESULTS OF THE LCA – additional impact categories according to EN 15804+A2-optional:
1 piece EntriWorX Unit 92 40
Parameter Unit A1-A3 A4 A5 B6 C2 C3 C4 D
Disease
PM 8.63E-07 2.2E-09 6.21E-10 2.56E-05 1.5E-11 2.46E-09 3.57E-11 -9.35E-08
incidence
IR kBq U235 eq 4.65E-01 1.32E-04 9.09E-04 1.16E+02 6.2E-06 1.68E-03 6.18E-06 -1.24E-01
ETP-fw CTUe 1.35E+02 6.08E-01 5.75E-02 2.28E+03 2.86E-02 1.89E-01 3.01E-03 -6.86E+00
HTP-c CTUh 1.91E-08 1.14E-11 3.36E-12 8.34E-08 5.39E-13 1.63E-11 4.47E-13 -4.78E-10
HTP-nc CTUh 2.96E-07 4.91E-10 1.92E-10 3.32E-06 2.3E-11 1.65E-09 4.92E-11 -3.26E-08
SQP SQP 7.6E+01 2.21E-03 3.44E-02 1.71E+03 1.04E-04 1.51E-01 1.1E-03 -6.06E+00
PM = Potential incidence of disease due to PM emissions; IR = Potential Human exposure efficiency relative to U235; ETP-fw = Potential comparative
Toxic Unit for ecosystems; HTP-c = Potential comparative Toxic Unit for humans (cancerogenic); HTP-nc = Potential comparative Toxic Unit for humans
(not cancerogenic); SQP = Potential soil quality index
Disclaimer 1 – for the indicator IRP This impact category deals mainly with the eventual impact of low dose ionizing radiation on human
health of the nuclear fuel cycle. It does not consider effects due to possible nuclear accidents, occupational exposure nor due to
radioactive waste disposal in underground facilities. Potential ionizing radiation from the soil, from radon and from some construction
materials is also not measured by this indicator.
Disclaimer 2 – for the indicators ADPE, ADPF, WDP, ETP-fw, HTP-c, HTP-nc, SQP
The results of this environmental impact indicator shall be used with care as the uncertainties on these results are high or as there is
limited experience with the indicator. This EPD was created using a software tool.
References
Standards (EAS), Radio Frequency Identification (RFID) and similar
applications.
CAN/CSA-22.2 No. 62368-1
CAN/CSA-22.2 No. 62368-1:2014, Audio/video, information and EN 55024+A1
communication technologyequipment — Part 1: Safety EN 55024:2010+A1:2015, Information technology equipment -
requirements. Immunity characteristics - Limits and methods of measurement.
Electromagnetic Compatibility Directive (EMC) EN 55032
Directive 2014/30/EU of the European Parliamant and of the EN 55032:2015, Electromagnetic compatibility of multimedia
Council of 26 February 2014 on the harmonisation of the laws equipment - Emission Requirements.
of the Member
States relating to electromagnetic compatibility. EN 60529
EN 60529:2014, Degrees of protection provided by enclosures
EN 15804+A2 (IP 20).
EN 15804:2019+A2 (in press), Sustainability of construction
works — Environmental Product Declarations — Core rules for EN 62368-1+A11
the product category of construction products. EN 62368-1:2014+A11:2017, Audio/video, information and
communication technology equipment - Part 1: Safety
EN 300330 V2.1.1 requirements.
Short Range Devices (SRD) - Radio equipment in the
frequency range 9 kHz to 25 MHz and inductive loop systems in ISO 14025
the frequency range 9 kHz to 30 MHz - Harmonised Standard DIN EN ISO 14025:2011-10, Environmental labels and
covering the essential requirements of article 3.2 of the declarations — Type III environmental declarations —
Directive 2014/53/EU. Principles and procedures.
EN 301489-1 V2.2.1 Low Voltage Directive (LVD)
ElectroMagnetic Compatibility (EMC) standard for radio Directive 2014/35/EU of the European Parliament and of the
equipment and services - Part 1: Common technical Council of 26 February 2014 on the harmonisation of the laws
requirements - Harmonised Standard covering the essential of the Member States relating to the making available on the
requirements of article 3.1(b) of Directive 2014/53/EU and the market of electrical equipment designed for use within certain
essential requirements of article 6 of Directive 2014/30/EU. voltage limits.
EN 301489-3 V2.1.1 Radio Equipment Directive (RED)
ElectroMagnetic Compatibility (EMC) standard for radio Directive 2014/53/EU of the European Parliament and of the
equipment and services - Part 3: Specific conditions for Short- Council of 16 April 2014 on the harmonisation of the laws of the
Range Devices (SRD) operating on frequencies between 9 kHz Member States relating to the making available on the market
and 246 GHz - Harmonised standard covering the essential of radio equipment and repealing Directive 1999/5/EC.
requirements of article 3.1(b) of Directive 2014/53/EU.
Registration, Evaluation, Authorisation and Restriction of
EN 50364 Chemicals (REACH)
EN 50364:2010, Limitation of human exposure to Regulation (EC) No 1907/2006 of the European Parliament and
electromagnetic fields from devices operating in the frequency of the Council on the Registration, Evaluation, Authorisation
range 0 Hz to 300 GHz, used in Electronic Article Surveillance and Restriction of Chemicals (REACH).
5 Environmental Product Declaration - dormakaba - EntriWorX Unit 92 40
GaBi ts software
Restriction of Hazardous Substances (RoHS) Sphera Solutions GmbH Gabi Software System and Database
Directive on the restriction of the use of certain hazardous for Life Cycle Engineering 1992-2020 Version 10.0.0.71
substances in electrical and electronic equipment (RoHS), University of Stuttgart Leinfelden-Echterdingen
Directive (EU) No 2011/65.
GaBi ts documentation
UL 294 GaBi life cycle inventory data documentation (https://www.gabi-
UL 294:2013, Standard for Safety Access Control System Unit. software.com/support/gabi/gabi-database-2020-lci-
documentation/).
UL 62368-1
UL 62368-1:2014, Standard for Audio/video, information and LCA-tool dormakaba
communication technology equipment - Part 1: Safety LCA tool, version 1.0. Developed by Sphera Solutions GmbH.
requirements.
PCR Part A
Further References PCR – Part A:
Calculation Rules for the Life Cycle As-sessment and
IBU 2021 Requirements on the Project Re-port according to EN
Institut Bauen und Umwelt e.V.: General Instructions for the 15804+A2:2019, Version 1.0, Institut Bauen und Umwelt e.V.,
EPD programme of Institut Bauen und Umwelt e.V. Version www.ibu-epd.com.
2.0., Berlin: Institut Bauen und Umwelt e.V., 2021. www.ibu-
epd.com PCR Part B
PCR – Part B: Requirements on the EPD for Electronic and
physical Access Control Systems, version 08/2021, Institut
Bauen und Umwelt e.V., www.ibu-epd.com.
6 Environmental Product Declaration - dormakaba - EntriWorX Unit 92 40
Publisher
Institut Bauen und Umwelt e.V. +49 (0)30 3087748- 0
Hegelplatz 1 info@ibu-epd.com
10117 Berlin www.ibu-epd.com
Germany
Programme holder
Institut Bauen und Umwelt e.V. +49 (0)30 3087748- 0
Hegelplatz 1 info@ibu-epd.com
10117 Berlin www.ibu-epd.com
Germany
Author of the Life Cycle Assessment
Sphera Solutions GmbH +49 711 341817-0
Hauptstraße 111- 113 info@sphera.com
70771 Leinfelden-Echterdingen www.sphera.com
Germany
Owner of the Declaration
dormakaba International Holding GmbH +49 2333 793-0
DORMA Platz 1 info.de@dormakaba.com
58256 Ennepetal www.dormakaba.com
Germany
7 Environmental Product Declaration - dormakaba - EntriWorX Unit 92 40
