ENVIRONMENTAL PRODUCT DECLARATION
as per ISO 14025 and EN 15804+A2
Owner of the Declaration dormakaba International Holding GmbH
Publisher Institut Bauen und Umwelt e.V. (IBU)
Programme holder Institut Bauen und Umwelt e.V. (IBU)
Declaration number EPD-DOR-20210335-CBA6-EN
Issue date 04.05.2022
Valid to 03.05.2027
BEST 45H Mortise Series
dormakaba
www.ibu-epd.com | https://epd-online.com
General Information
dormakaba BEST 45H Mortise Series
Programme holder Owner of the declaration
IBU – Institut Bauen und Umwelt e.V. dormakaba International Holding GmbH
Hegelplatz 1 DORMA Platz 1
10117 Berlin 58256 Ennepetal
Germany Germany
Declaration number Declared product / declared unit
EPD-DOR-20210335-CBA6-EN 1 mortise lock (1 piece) of the BEST 45H Series.
This declaration is based on the product category rules: Scope:
Building Hardware products, 01.08.2021 This Environmental Product Declaration refers to a specific lock
(PCR checked and approved by the SVR) manufactured by dormakaba. The production site is located in Indianapolis
(USA).
Issue date The data represents the year 2020.
The owner of the declaration shall be liable for the underlying information
04.05.2022
and evidence; the IBU shall not be liable with respect to manufacturer
information, life cycle assessment data and evidences.
Valid to
The EPD was created according to the specifications of EN 15804+A2. In
03.05.2027 the following, the standard will be simplified as EN 15804.
Verification
The standard EN 15804 serves as the core PCR
Independent verification of the declaration and data according to ISO
14025:2011
internally X externally
Dipl.-Ing. Hans Peters
(Chairman of Institut Bauen und Umwelt e.V.)
Florian Pronold Dr.-Ing. Wolfram Trinius,
(Managing Director Institut Bauen und Umwelt e.V.) (Independent verifier)
1 Environmental Product Declaration - dormakaba - BEST 45H Mortise Series
Product
Performance data of the product with respect
Product description/Product definition to its characteristics in accordance with the
BEST’s 45H series mortise locks deliver exceptional strength, relevant technical provision which can be applied are
security, and durability. The robust design features and mentioned
precision-engineered components make the 45H mortise lock above.
series ideal for high traffic applications. Backed by an industry-
leading limited lifetime mechanical warranty, the 45H series Base materials/Ancillary materials
delivers security you can depend on. For the use and The major material compositions including the packaging of the
application of the product the respective national provisions at product are listed below:
the place of use apply. The standards which can be applied are Name Value Unit
the following:
Brass 50 %
• ANSI/BHMA A156.13 Steel 29 %
• ANSI A117.1 (Accessibility, ADA compliant)
Stainless steel 11 %
• Florida Building Code (FBC) listed
Electronics 5 %
• Miami-Dade County Code compliant
• UL listed Zinc 4 %
Plastics 1 %
Application
Other materials <1 %
The 45H Mortise Series can be used for following building
types: The product/s include/s partial articles which contain
substances listed in the Candidate List of REACH Regulation
• Learning and higher education
1907/2006/EC (date: 17.01.2022) exceeding 0.1 percentage by
• Healthcare
mass: yes
• Government
• Retail and commercial
• Lead (Pb): 7439-92-1 (CAS-No.) is included in some of
Technical Data the alloys used. The concentration of lead in each
The lock has following technical properties: individual alloy does not exceed 4.0% (by mass).
The Candidate List can be found on the ECHA website
address: https://echa.europa.eu/de/home.
Reference service life
The reference service life of the 45H Mortise Series lock
depends on the traffic pattern and degree of usage of the door.
These locks are rated to ANSI Grade 1, meaning they are
designed to withstand a minimum of 1,000,000 cycles.
However, the 45H Mortise lock has been independently tested
to surpass 10,000,000 cycles.
LCA: Calculation rules
— A3, manufacturing and assembly including provision of all
Declared Unit materials, products and energy, as well as waste processing up
The declared unit is 1 piece of the product: BEST 45H Mortise to the end-of waste state.
Series.
Name Value Unit Construction stage - Modules A4-A5
Declared unit 1 piece/product The construction process stage includes:
— A4, transport to the building site;
Mass of declared Product 3.8 kg
— A5, installation into the building; including provision of all
materials, products and energy, as well as waste processing up
System boundary
to the end-of waste state or disposal of final residues during the
The type of EPD is: cradle to gate with options, modules C1–
construction process stage.
C4, and module D (A1–A3 + C + D and additional modules: A4
+ A5)
End-of-life stage– Modules C1-C4 and D
The end-of-life stage includes:
Production - Module A1-A3
— C1, de-construction, demolition:
The product stage includes:
— C2, transport to waste processing;
— A1, raw material extraction, processing and mechanical
— C3, waste processing for reuse, recovery and/or recycling;
treatments, processing of secondary material input (e.g.
— C4, disposal; including provision and all transport, provision
recycling processes),
of all materials, products and related energy and water use.
— A2, transport to the manufacturer,
2 Environmental Product Declaration - dormakaba - BEST 45H Mortise Series
— Module D (Benefits and loads beyond the system boundary)
includes: Comparability
— D, recycling potentials, expressed as net impacts and Basically, a comparison or an evaluation of EPD data is only
benefits. possible if all the data sets to be compared were created
according to EN 15804 and the building context, respectively
Geographic Representativeness the product-specific characteristics of performance, are taken
Land or region, in which the declared product system is into account.
manufactured, used or handled at the end of the product´s
lifespan: United States
LCA: Scenarios and additional technical information
Operational energy use (B6)
Characteristic product properties of biogenic carbon
Name Value Unit
Information on describing the biogenic Carbon Content at
Electricity consumption for 1 year 28.47 kWh
factory gate
Power consumption "on mode" 78 W
Name ValueUnit
Hours per day in use "on mode" 1 h
kg
Biogenic carbon content in product - C Power consumption "standby mode" 0 W
Biogenic carbon content in accompanying kg Hours per day in use "standby mode" 23 h
-
packaging C
End of life (C1-C4)
C1: The product dismantling from the building is done manually
Additional technical information for the declared modules. without environmental burden.
Transport to the building site (A4) C2: Transport to waste treatment at end of life is 50km.
Name Value Unit Name Value Unit
Litres of fuel per 1 kg (truck) 0.00276l/100km Collected separately waste type 3.8 kg
Transport distance (truck) 1500 km Recycling 3.58 kg
Capacity utilisation (including empty runs) Energy recovery 0.024 kg
55 %
average Final desposition 0,201 kg
Transport distance (ship) 10000 km
Reuse, recovery and/or recycling potentials (D), relevant
Installation into the building (A5) scenario information
Name Value Unit Name Value Unit
Output substances following waste treatment on Recycling 100 %
0.00017 kg
site (packaging)
Collection rate is 100%.
3 Environmental Product Declaration - dormakaba - BEST 45H Mortise Series
LCA: Results
DESCRIPTION OF THE SYSTEM BOUNDARY (X = INCLUDED IN LCA; MND = MODULE OR INDICATOR NOT DECLARED; MNR
= MODULE NOT RELEVANT)
Benefits and
Construction loads beyond
Product stage Use stage End of life stage
process stage the system
boundaries
la ire ta m w a Ry lp p u s tro p s n a rT g n iru tc a fu n a M e h t m o rf tro p s n a rTe tis e h t o t e ta g y lb m e s s A e s U e c n a n e tn ia M ria p e R tn e m e c a lp e R tn e m h s ib ru fe R y g re n e la n o ita re p Oe s u re ta w la n o ita re p Oe s u n o itc u rts n o c -e Dn o itilo m e d tro p s n a rT g n is s e c o rp e ts a W la s o p s iD -e s u e R-y re v o c e R-g n ilc y c e Rla itn e to p
A1 A2 A3 A4 A5 B1 B2 B3 B4 B5 B6 B7 C1 C2 C3 C4 D
X X X X X MND MND MNR MNR MNR X MND X X X X X
RESULTS OF THE LCA - ENVIRONMENTAL IMPACT according to EN 15804+A2: 1 mortise lock
Parameter Unit A1-A3 A4 A5 B6 C1 C2 C3 C4 D
GWP-total kg CO 2 eq 9.94E+00 6.23E-01 2.41E-04 0 0 1.7E-02 6.3E-02 3E-03 -3.28E+00
GWP-fossil kg CO 2 eq 9.87E+00 6.01E-01 6.04E-06 0 0 1.6E-02 6.3E-02 3E-03 -3.29E+00
GWP-biogenic kg CO 2 eq 5.3E-02 2.2E-02 2.35E-04 0 0 7.32E-04 1.47E-06 1.04E-05 6E-03
GWP-luluc kg CO 2 eq 1.15E-02 1.39E-05 3.97E-09 0 0 3.77E-07 3.58E-06 8.78E-06 -3E-03
ODP kg CFC11 eq 1.03E-11 6.21E-17 4.34E-20 0 0 1.67E-18 3.19E-17 1.13E-17 -2.37E-15
AP mol H+ eq 5.2E-02 5E-03 6.75E-08 0 0 1.58E-05 1.13E-05 2.19E-05 -1E-02
EP-freshwater kg P eq 1.45E-05 1.3E-07 8.5E-12 0 0 3.39E-09 5.09E-09 5.24E-09 -2.95E-06
EP-marine kg N eq 7.25E-03 1E-03 2.44E-08 0 0 5.04E-06 2.54E-06 5.63E-06 -2E-03
EP-terrestrial mol N eq 7.5E-02 1.5E-02 3.04E-07 0 0 5.6E-05 5.13E-05 6.19E-05 -2E-02
kg NMVOC
POCP 2.17E-02 4E-03 6.46E-08 0 0 1.43E-05 7.03E-06 1.71E-05 -6E-03
eq
ADPE kg Sb eq 2.04E-03 1.75E-08 6.86E-13 0 0 4.75E-10 4.38E-10 2.74E-10 3.22E-05
ADPF MJ 1.23E+02 8.27E+00 7.61E-05 0 0 2.24E-01 2.9E-02 4E-02 -3.57E+01
m3 world eq
WDP 2.15E+00 1E-03 2.99E-05 0 0 3.1E-05 6E-03 3.2E-04 -8.24E-01
deprived
GWP = Global warming potential; ODP = Depletion potential of the stratospheric ozone layer; AP = Acidification potential of land and water; EP =
Eutrophication potential; POCP = Formation potential of tropospheric ozone photochemical oxidants; ADPE = Abiotic depletion potential for non-fossil
resources; ADPF = Abiotic depletion potential for fossil resources; WDP = Water (user) deprivation potential)
RESULTS OF THE LCA - INDICATORS TO DESCRIBE RESOURCE USE according to EN 15804+A2: 1 mortise lock
Parameter Unit A1-A3 A4 A5 B6 C1 C2 C3 C4 D
PERE MJ 2.48E+01 2.6E-02 2E-03 0 0 7.08E-04 2.1E-02 5E-03 -4.26E+00
PERM MJ 1.5E-02 0 -2E-03 0 0 0 -1.3E-02 0 0
PERT MJ 2.48E+01 2.6E-02 1.38E-05 0 0 7.08E-04 8E-03 5E-03 -4.26E+00
PENRE MJ 1.22E+02 8.28E+00 7.61E-05 0 0 2.25E-01 8.41E-01 4E-02 -3.58E+01
PENRM MJ 8.11E-01 0 0 0 0 0 -8.11E-01 0 0
PENRT MJ 1.23E+02 8.28E+00 7.61E-05 0 0 2.25E-01 2.9E-02 4E-02 -3.58E+01
SM kg 2.61E+00 0 0 0 0 0 0 0 0
RSF MJ 0 0 0 0 0 0 0 0 0
NRSF MJ 0 0 0 0 0 0 0 0 0
FW m3 6.91E-02 4.72E-05 7.04E-07 0 0 1.27E-06 1.55E-04 1.01E-05 -3.3E-02
PERE = Use of renewable primary energy excluding renewable primary energy resources used as raw materials; PERM = Use of renewable primary
energy resources used as raw materials; PERT = Total use of renewable primary energy resources; PENRE = Use of non-renewable primary energy
excluding non-renewable primary energy resources used as raw materials; PENRM = Use of non-renewable primary energy resources used as raw
materials; PENRT = Total use of non-renewable primary energy resources; SM = Use of secondary material; RSF = Use of renewable secondary fuels;
NRSF = Use of non-renewable secondary fuels; FW = Use of net fresh water
RESULTS OF THE LCA – WASTE CATEGORIES AND OUTPUT FLOWS according to EN 15804+A2:
1 mortise lock
Parameter Unit A1-A3 A4 A5 B6 C1 C2 C3 C4 D
HWD kg 3.79E-07 8.05E-10 1.12E-13 0 0 2.18E-11 1.12E-10 6.1E-10 -1.57E-06
NHWD kg 9.16E-01 8.47E-04 7.55E-06 0 0 2.3E-05 7E-03 2.01E-01 -1.9E-02
RWD kg 4.97E-03 8.95E-06 4E-09 0 0 2.41E-07 1.09E-06 4.56E-07 -2.93E-04
CRU kg 0 0 0 0 0 0 0 0 0
MFR kg 0 0 0 0 0 0 3.56E+00 0 0
MER kg 0 0 0 0 0 0 0 0 0
EEE MJ 1.7E-02 0 3.65E-04 0 0 0 0 0 0
EET MJ 3.1E-02 0 6.61E-04 0 0 0 0 0 0
HWD = Hazardous waste disposed; NHWD = Non-hazardous waste disposed; RWD = Radioactive waste disposed; CRU = Components for re-use;
MFR = Materials for recycling; MER = Materials for energy recovery; EEE = Exported electrical energy; EET = Exported thermal energy
4 Environmental Product Declaration - dormakaba - BEST 45H Mortise Series
RESULTS OF THE LCA – additional impact categories according to EN 15804+A2-optional:
1 mortise lock
Parameter Unit A1-A3 A4 A5 B6 C1 C2 C3 C4 D
Disease
PM 5.96E-07 8.08E-08 3.74E-13 0 0 8.33E-11 1.44E-10 2.71E-10 -2.07E-07
incidence
IR kBq U235 eq 6.77E-01 1E-03 6.19E-07 0 0 3.45E-05 9.81E-05 4.69E-05 -2.3E-02
ETP-fw CTUe 6.6E+01 5.86E+00 3.61E-05 0 0 1.59E-01 1.1E-02 2.3E-02 -1.1E+01
HTP-c CTUh 5.9E-07 1.1E-10 1.91E-15 0 0 2.99E-12 9.53E-13 3.39E-12 -1.4E-09
HTP-nc CTUh 2.46E-07 4.81E-09 8.28E-14 0 0 1.28E-10 9.65E-11 3.74E-10 2.03E-07
SQP SQP 2.83E+01 2.1E-02 2.02E-05 0 0 5.77E-04 9E-03 8E-03 -1.47E+00
PM = Potential incidence of disease due to PM emissions; IR = Potential Human exposure efficiency relative to U235; ETP-fw = Potential comparative
Toxic Unit for ecosystems; HTP-c = Potential comparative Toxic Unit for humans (cancerogenic); HTP-nc = Potential comparative Toxic Unit for humans
(not cancerogenic); SQP = Potential soil quality index
Disclaimer 1 – for the indicator “Potential Human exposure efficiency relative to U235”. This impact category deals mainly with the
eventual impact of low-dose ionizing radiation on human health of the nuclear fuel cycle. It does not consider effects due to possible
nuclear accidents, occupational exposure or radioactive waste disposal in underground facilities. Potential ionizing radiation from the
soil, radon and from some construction materials is also not measured by this indicator.
Disclaimer 2 – for the indicators “abiotic depletion potential for non-fossil resources”, “abiotic depletion potential for fossil resources”,
“water (user) deprivation potential, deprivation-weighted water consumption”, “potential comparative toxic unit for ecosystems”,
“potential comparative toxic unit for humans – cancerogenic”, “Potential comparative toxic unit for humans - not cancerogenic”,
“potential soil quality index”. The results of this environmental impact indicator shall be used with care as the uncertainties on these
results are high as there is limited experience with the indicator.
References
ADA (version 1-6) Gabi Software System and Database for Life Cycle
Americans with Disabilities Act 1990. Engineering 1992-2020
Version 10.0.0.71
ANSI A117.1 University of Stuttgart
ANSI A117.1-2017: Accessible and Usable Buildings. Leinfelden-Echterdingen.
ANSI/BHMA A156.13 GaBi ts documentation
ANSI/BHMA A1564.13:2017 - Mortise Locks. GaBi life cycle inventory data documentation (https://www.gabi-
software.com/support/gabi/gabidatabase-
2020-lci-documentation/).
EN 15804
EN 15804:2019+A2, Sustainability of construction works — LCA-tool dormakaba
Environmental Product Declarations — Core rules for the LCA-tool, IBU-DOR-202104-LT1-EN. Developed by Sphera
product category of construction products. Solutions GmbH.
REACH Regulation 1907/2006/EC Miami-Dade County Code
Regulation (EC) No 1907/2006 of the European https://www.miamidade.gov/cob/ordinances-enacted-by-
Parliament and of the Council on the Registration, bcc.asp.
Evaluation, Authorisation and Restriction of Chemicals
(REACH). PCR Part A
PCR – Part A: Calculation Rules for the Life Cycle Assessment
Further References and Requirements on the Project Re-port
according to EN 15804+A2:2019, Version 1.0, 2020, Institut
Florida Building Code Bauen und Umwelt e.V., www.ibu-epd.com.
https://floridabuilding.org/c/default.aspx.
PCR Part B
IBU 2021 PCR – Part B: Requirements on the EPD for Building Hardware
Institut Bauen und Umwelt e.V.: General Instructions for the product, version, Institut Bauen und
EPDs programme of Institut Bauen und Umwelt e.V. Version Umwelt e.V., www.ibu-epd.com.
2.0., Berlin: Institut Bauen und Umwelt e.V., 2021. www.ibu-
epd.com. UL
Underwriters Laboratories,
GaBi https://www.ul.com/.
Sphera Solutions GmbH
5 Environmental Product Declaration - dormakaba - BEST 45H Mortise Series
Publisher
Institut Bauen und Umwelt e.V. +49 (0)30 3087748- 0
Hegelplatz 1 info@ibu-epd.com
10117 Berlin www.ibu-epd.com
Germany
Programme holder
Institut Bauen und Umwelt e.V. +49 (0)30 3087748- 0
Hegelplatz 1 info@ibu-epd.com
10117 Berlin www.ibu-epd.com
Germany
Author of the Life Cycle Assessment
Sphera Solutions GmbH +49 711 341817-0
Hauptstraße 111- 113 info@sphera.com
70771 Leinfelden-Echterdingen www.sphera.com
Germany
Owner of the Declaration
dormakaba International Holding GmbH +49 2333 793-0
DORMA Platz 1 info.de@dormakaba.com
58256 Ennepetal www.dormakaba.com
Germany
6 Environmental Product Declaration - dormakaba - BEST 45H Mortise Series
