ENVIRONMENTAL PRODUCT DECLARATION
as per ISO 14025 and EN 15804+A2
Owner of the Declaration Knauf Ceiling Solutions GmbH & Co. KG
Publisher Institut Bauen und Umwelt e.V. (IBU)
Programme holder Institut Bauen und Umwelt e.V. (IBU)
Declaration number EPD-KNA-20240025-IBI1-EN
Issue date 12.03.2024
Valid to 11.03.2029
Classic Max
Knauf Ceiling Solutions GmbH & Co. KG
www.ibu-epd.com | https://epd-online.com
1. General Information
Knauf Ceiling Solutions GmbH & Co. KG Classic Max
Programme holder Owner of the declaration
IBU – Institut Bauen und Umwelt e.V. Knauf Ceiling Solutions GmbH & Co. KG
Hegelplatz 1 Elsenthal 15
10117 Berlin 94481 Grafenau
Germany Germany
Declaration number Declared product / declared unit
EPD-KNA-20240025-IBI1-EN 1 m² Classic Max mineral ceiling tiles with a surface weight of 3.76 kg/m².
This declaration is based on the product category rules: Scope:
Mineral panels, 01.08.2021 This document refers to 1 m² Classic Max mineral ceiling tiles with a
(PCR checked and approved by the SVR) surface weight of 3.76 kg/m², manufactured at the production facility in
Wujiang, China.
Issue date The owner of the declaration shall be liable for the underlying information
and evidence; the IBU shall not be liable with respect to manufacturer
12.03.2024
information, life cycle assessment data and evidences.
The EPD was created according to the specifications of EN 15804+A2. In
Valid to
the following, the standard will be simplified as EN 15804.
11.03.2029
Verification
The standard EN 15804 serves as the core PCR
Independent verification of the declaration and data according to ISO
14025:2011
internally X externally
Dipl.-Ing. Hans Peters
(Chairman of Institut Bauen und Umwelt e.V.)
Florian Pronold Vito D'Incognito,
(Managing Director Institut Bauen und Umwelt e.V.) (Independent verifier)
1 Environmental Product Declaration - Knauf Ceiling Solutions GmbH & Co. KG - Classic Max
2. Product
This product/article/at least one partial article contains other
2.1 Product description/Product definition carcinogenic, mutagenic, reprotoxic (CMR) substances in
The ceiling tiles are manufactured using a wet-felt process and categories 1A or 1B which are not on the candidate list,
consist of biosoluble mineral wool, perlite, clay and starch. In exceeding 0.1 percentage by mass: No.
addition, the visible side of the mineral tile is painted with
dispersion paint. The back side is primed with dispersion paint. Biocide products were added to this construction product or it
has been treated with biocide products (this then concerns a
The mineral tiles are available in different formats and edge treated product as defined by the (EU) Ordinance on Biocide
finishes. Products No. 528/2012): No.
This EPD applies to the following products: In-can preservatives are used in the production process;
Classic Max however, they are not part of the products and are therefore not
within the scope of the Ordinance on Biocide Products.
For the use and application of the product, the respective
national provisions at the place of use apply, in Germany for 2.6 Manufacture
example the building codes of the federal states and the The mineral tiles are produced in the traditional wet process
corresponding national specifications. (wet-felt). The raw materials are mixed with water to form a
homogeneous suspension, which is pumped onto a belt
2.2 Application conveyor (Fourdrinier). The water is removed mechanically
Mineral tiles (wet-felt) are typically used as lay-in for suspended (gravity and vacuum) and by evaporation in the drying oven. As
ceiling constructions. They are primarily used as optical far as possible, the process water is reused. It is treated
cladding, but also for sound absorption and sound insulation, accordingly and fed back into the process water circuit.
for fire resistance and against fire spreading, for cleanrooms Production waste and dust are reused in the process in the
and high hygiene requirements. sense of an internal cycle. The manufacturing plant is certified
according to ISO 9001, ISO 14001 and ISO 45001.
2.3 Technical Data
2.7 Environment and health during manufacturing
Construction data • The manufacturing plant is certified according to ISO
Name Value Unit 9001, ISO 14001 and ISO 45001.
• The production has a closed water cycle.
Noise reduction coefficient acc. ISO 354
0.70 • Production generates almost no waste, resulting blanks,
and ASTM C 423-01
dust and rejects are reused.
Airborne Sound Attenuation acc. ISO 10848
30 dB • Not subject to declaration according to REACH.
and ASTM E1414
Formaldehyde after 52 h < 0.005 mg/m³ 2.8 Product processing/Installation
TVOC after 72 h 0.065 mg/(m²*h) There are no recognised systemic hazards associated with the
installation of ceiling tiles. It is recommended that materials are
handled in a manner that minimises dust generation. Workers
Performance data of the product with respect to its
should wear appropriate personal protective equipment.
characteristics in accordance with the relevant technical
Equipment such as gloves, goggles and dust masks are
provision (no CE-marking).
recommended to minimise exposure to dust and prevent skin
2.4 Delivery status irritation.
The EPD refers to panels with a thickness of 17mm which can
2.9 Packaging
have variable length and width dimensions.
The panels are packaged in cardboard boxes and sealed with
2.5 Base materials/Ancillary materials transparent polyethylene film. These packages lie on
chemically untreated wooden pallets. The pallets are wrapped
Mineral tile composition:
with polyethylene stretch film. Foil, paper and wood can be
Name Value Unit recycled in the usual ways.
Mineral wool 43 %
2.10 Condition of use
Perlite 18 %
When handled properly, the mechanical and structural-physical
Clay 0 %
properties of the mineral tile remain intact throughout its entire
Paper 8 % service life. Direct contact with water should be avoided due to
Starch 5 % the water-soluble binding agent starch.
Brokes/dust (internally looped production waste) 26 %
2.11 Environment and health during use
When properly installed, no dust/particles are released during
In addition, the visible side of the mineral tile is painted with the use phase. For the substance groups formaldehyde, volatile
dispersion paint. The back side is primed with a dispersion organic compounds (VOCs) and total volatile organic
paint. compounds (TVOCs), the limits according to GB/T 17657-2013
The recycled content is not less than 51 %. and HJ 571-2010 are complied with.
This product/article/at least one partial article contains 2.12 Reference service life
substances listed in the ECHA-candidate list (date: 25.06.2020) The service life of the mineral tiles (wet-felted) is up to
exceeding 0.1 percentage by mass: No. 50 years, depending on the area of use, exposure and state of
maintenance. Within the framework of the conditions of use, no
2 Environmental Product Declaration - Knauf Ceiling Solutions GmbH & Co. KG - Classic Max
ageing effects are to be expected apart from visual Mechanical destruction
discolouration caused by air circulation. The mineral slabs (wet-felt) can be broken by hand and also
damaged superficially, which can result in minor dust formation.
2.13 Extraordinary effects
Fire 2.14 Re-use phase
If the panels are removed properly, they can be reinstalled. In
The declared products are classified in the fire reaction class 0 case of minor damage, the slabs can be reused as cut-to-size
according to BS 476 Part 6. tiles. Mineral tiles can be returned to the manufacturing process
Name Value if they are of the correct type and have sufficient material
quality; they can be recycled up to 100 %.
Building material class acc. ASTM E84 Class A
Building material class acc. BS 476 Part 6&7 Class 0 2.15 Disposal
The waste code number of production residues for mineral tiles
Water according to the AVV, German List of Wastes Ordinance is 10
In the case of prolonged contact with water, the starch binder 11 03, the waste code number for construction site waste
dissolves, which can lead to a loss of structure, and if the (offcuts) is 17 06 04. If the tiles are not recycled as described in
soluble components are discharged into the sewage treatment 2.14., they are disposed of in a landfill.
plant, they are biodegradable, increasing the chemical oxygen
2.16 Further information
demand (COD) and biological oxygen demand (BOD).
Further information at www.knaufceilingsolutions.com
3. LCA: Calculation rules
C4.
3.1 Declared Unit
This EPD refers to a declared unit of 1 m² Classic Max mineral Module C4 | Disposal
ceiling tiles with a surface weight of 3.76 kg/m². Module C4 refers to the emissions from the disposal of the
Declared Unit acoustic board mineral ceiling tiles. The chosen scenario,
therefore, includes the environmental burdens of landfilling the
Name Value Unit
product.
Declared unit 1 m2
Grammage (with coating) 3.76 kg/m2 Module D | Benefits and loads beyond the system
Layer thickness 0.017 m boundary
The declared scenario assumes landfilling of the product.
Boardmill density (raw board, without coating) 210 kg/m³
Referring environmental impacts are accounted for in module
C4.
The ceiling tiles are produced at the Knauf Ceiling Solutions
production site in Wujiang, China. 3.3 Estimates and assumptions
Various types of mineral ceiling tiles are produced at the site. Assumptions and approximations are applied in case of a lack
of representative data. All assumptions and approximations are
3.2 System boundary documented precisely and represent a best-guess
The life cycle assessment of Classic Max mineral ceiling tiles representation of reality. In case of uncertainty, a conservative
includes a cradle-to-gate analysis of the products' approach is chosen.
environmental impacts with modules (A1–A3, C, D).
Subsequent life cycle phases are part of the analysis: This study builds on Chinese background data as far as
supported by the available databases. Nevertheless, some
Module A1–A3 | Production stage upstream supply chains of used raw materials were
The production stage includes the upstream burdens of raw approximated via European data, due to a lack of
material supply, their transports and the manufacturing plant of geographically adapted datasets.
Knauf Ceiling Solutions located in Wujiang (China). Mineral
ceiling tiles are produced in the wet-felt process. Main raw 3.4 Cut-off criteria
material inputs, therefore, refer to mineral wool, perlite, clay and The LCA model covers all available input and output flows,
starch. The production site is supplied with electricity from the which can be represented based on robust data. Data gaps are
Chinese power grid and thermal energy from natural gas. filled with conservative assumptions from average data (when
available) or with generic data and are documented
Module C1 | Deconstruction and demolition accordingly. Only data with a contribution lower than 1 % were
Disassembly of the product is done either manually or using cut off. Thus, no data were neglected, of which a substantial
smaller tools. Referring energy demand is considered to be impact is to be expected. All relevant data were collected
negligible. comprehensively. Cut-off material and energy flows were
chosen carefully based on their expected quantitative
Modul C2 | Transport to disposal contribution as well as potential environmental impacts. Thus, it
The transport to the disposal of the material is estimated can be assumed that the sum of all neglected input flows does
declaring a 50 km radius to the landfill. In reality, this scenario not account for more than 5 % of the total material, water and
may vary depending on the actual location of deconstruction energy flows.
and referring waste treatment.
3.5 Background data
Module C3 | Waste processing This study uses generic background data for the evaluation of
The declared scenario assumes landfilling of the product. upstream environmental impacts from GaBi databases (GaBi
Referring environmental impacts are accounted for in module 10; 2022.2).
3 Environmental Product Declaration - Knauf Ceiling Solutions GmbH & Co. KG - Classic Max
3.6 Data quality 3.9 Allocation
Data collection is based on product-specific questionnaires. It All information for the allocation of given material and energy
follows an iterative process of clarifying questions via e-mail, flows is based on site-related evaluations. The calculation of
telephone calls or in personal/web meetings. Intensive specific input quantities for the raw board production is based
discussions between Knauf Ceiling Solutions and Daxner & on the respective recipe. In addition, product-specific
Merl result in an accurate mapping of product-related material application rates (e.g. backcoat, primer, etc.) were available.
and energy flows. This leads to a high quality of foreground Total annual energy consumption and waste flows are allocated
data collected. Data collection relies on a consistent process based on the production share of the product.
according to ISO 14044.
For in the production used waste paper, the system boundary is
The technological, geographical and time-related set after sorting. It is assumed that the end-of-waste status has
representativeness of the database was kept in mind when been reached. The system boundary for secondary raw
selecting background data. Whenever specific data were materials defined in EN 15804 applies.
missing, either generic datasets or representative average data
were used instead. The implemented GaBi background 3.10 Comparability
datasets refer to the latest versions available (not more than Basically, a comparison or an evaluation of EPD data is only
ten years old) and are carefully chosen. possible if all the data sets to be compared were created
according to EN 15804 and the building context, respectively
3.7 Period under review the product-specific characteristics of performance, are taken
Foreground data were collected in the 2021 production year, into account.
and the data are based on the volumes produced on an annual
basis. The GaBi background database was used to calculate the LCA
(GaBi 10; 2022.2).
3.8 Geographic Representativeness
Land or region, in which the declared product system is
manufactured, used or handled at the end of the product´s
lifespan: China
4. LCA: Scenarios and additional technical information
Characteristic product properties of biogenic carbon
The biogenic carbon content quantifies the amount of biogenic
carbon in the declared product.
Installation in building (A5)
Information on the description of the biogenic carbon The End-of-Life of the product packaging materials is not
content at the factory gate declared in module A5.
Name ValueUnit Name Value Unit
Biogenic carbon content in product 0.26 kg Packaging (cardboard) 0.009 kg/m²
C
Packaging (PE-film) 0.035 kg/m²
Biogenic carbon content in accompanying kg
0.015
packaging C
End-of-Life (C1–C4)
The carbon stored in the packaging was taken into account as Name Value Unit
"CO 2-neutral". Thus the storage effect of the carbon bound in Collected separately 3.76 kg
the packaging is not included in the calculation but is Landfilling 3.76 kg
considered as emitted immediately.
4 Environmental Product Declaration - Knauf Ceiling Solutions GmbH & Co. KG - Classic Max
5. LCA: Results
The following table contains the LCA results for a declared unit of 1 m² Classic Max mineral ceiling tiles with a surface weight of
3.76 kg/m².
DESCRIPTION OF THE SYSTEM BOUNDARY (X = INCLUDED IN LCA; MND = MODULE OR INDICATOR NOT DECLARED; MNR
= MODULE NOT RELEVANT)
Benefits and
Construction loads beyond
Product stage Use stage End of life stage
process stage the system
boundaries
la ire ta m w a Ry lp p u s tro p s n a rT g n iru tc a fu n a M e h t m o rf tro p s n a rTe tis e h t o t e ta g y lb m e s s A e s U e c n a n e tn ia M ria p e R tn e m e c a lp e R tn e m h s ib ru fe R y g re n e la n o ita re p Oe s u re ta w la n o ita re p Oe s u n o itc u rts n o c -e Dn o itilo m e d tro p s n a rT g n is s e c o rp e ts a W la s o p s iD -e s u e R-y re v o c e R-g n ilc y c e Rla itn e to p
A1 A2 A3 A4 A5 B1 B2 B3 B4 B5 B6 B7 C1 C2 C3 C4 D
X X X MND MND MND MND MNR MNR MNR MND MND X X X X X
RESULTS OF THE LCA - ENVIRONMENTAL IMPACT according to EN 15804+A2: 1 m² Classic Max ceiling tiles (3.76 kg/m²)
Parameter Unit A1-A3 C1 C2 C3 C4 D
Global Warming Potential total (GWP-total) kg CO 2 eq 1.84E+01 0 1.18E-02 0 1E+00 0
Global Warming Potential fossil fuels (GWP-fossil) kg CO 2 eq 1.93E+01 0 1.13E-02 0 5.61E-02 0
Global Warming Potential biogenic (GWP-biogenic) kg CO 2 eq -9.32E-01 0 4.99E-04 0 9.46E-01 0
Global Warming Potential luluc (GWP-luluc) kg CO 2 eq 1.33E-02 0 2.94E-07 0 1.04E-04 0
Depletion potential of the stratospheric ozone layer (ODP) kg CFC11 eq 1.34E-10 0 1.11E-15 0 1.32E-13 0
Acidification potential of land and water (AP) mol H+ eq 6.24E-02 0 3.79E-05 0 3.98E-04 0
Eutrophication potential aquatic freshwater (EP-freshwater) kg P eq 4.22E-05 0 1.42E-09 0 9.51E-08 0
Eutrophication potential aquatic marine (EP-marine) kg N eq 1.36E-02 0 1.72E-05 0 1.02E-04 0
Eutrophication potential terrestrial (EP-terrestrial) mol N eq 1.6E-01 0 1.89E-04 0 1.12E-03 0
Formation potential of tropospheric ozone photochemical oxidants kg NMVOC
4.42E-02 0 3.42E-05 0 3.09E-04 0
(POCP) eq
Abiotic depletion potential for non fossil resources (ADPE) kg Sb eq 2.8E-04 0 4.57E-10 0 5.75E-09 0
Abiotic depletion potential for fossil resources (ADPF) MJ 2.97E+02 0 1.56E-01 0 7.35E-01 0
m3 world eq
Water use (WDP) 5.59E+00 0 9.6E-05 0 6.15E-03 0
deprived
RESULTS OF THE LCA - INDICATORS TO DESCRIBE RESOURCE USE according to EN 15804+A2: 1 m² Classic Max ceiling
tiles (3.76 kg/m²)
Parameter Unit A1-A3 C1 C2 C3 C4 D
Renewable primary energy as energy carrier (PERE) MJ 1.11E+02 0 8.44E-04 0 1.1E-01 0
Renewable primary energy resources as material utilization
MJ 1.11E+01 0 0 0 0 0
(PERM)
Total use of renewable primary energy resources (PERT) MJ 1.22E+02 0 8.44E-04 0 1.1E-01 0
Non renewable primary energy as energy carrier (PENRE) MJ 2.97E+02 0 1.56E-01 0 7.36E-01 0
Non renewable primary energy as material utilization (PENRM) MJ 3.91E-01 0 0 0 0 0
Total use of non renewable primary energy resources (PENRT) MJ 2.97E+02 0 1.56E-01 0 7.36E-01 0
Use of secondary material (SM) kg 1.36E-01 0 0 0 0 0
Use of renewable secondary fuels (RSF) MJ 0 0 0 0 0 0
Use of non renewable secondary fuels (NRSF) MJ 0 0 0 0 0 0
Use of net fresh water (FW) m3 1.85E-01 0 2.42E-06 0 1.87E-04 0
RESULTS OF THE LCA – WASTE CATEGORIES AND OUTPUT FLOWS according to EN 15804+A2:
1 m² Classic Max ceiling tiles (3.76 kg/m²)
Parameter Unit A1-A3 C1 C2 C3 C4 D
Hazardous waste disposed (HWD) kg 1.54E-06 0 3.91E-13 0 3.78E-11 0
Non hazardous waste disposed (NHWD) kg 3.72E+00 0 6.47E-06 0 3.76E+00 0
Radioactive waste disposed (RWD) kg 1.21E-02 0 8.78E-08 0 8.17E-06 0
Components for re-use (CRU) kg 0 0 0 0 0 0
Materials for recycling (MFR) kg 0 0 0 0 0 0
Materials for energy recovery (MER) kg 0 0 0 0 0 0
Exported electrical energy (EEE) MJ 0 0 0 0 0 0
Exported thermal energy (EET) MJ 0 0 0 0 0 0
RESULTS OF THE LCA – additional impact categories according to EN 15804+A2-optional:
1 m² Classic Max ceiling tiles (3.76 kg/m²)
Parameter Unit A1-A3 C1 C2 C3 C4 D
Incidence of disease due to PM emissions (PM) Disease 6.3E-07 0 2.04E-10 0 4.9E-09 0
5 Environmental Product Declaration - Knauf Ceiling Solutions GmbH & Co. KG - Classic Max
incidence
Human exposure efficiency relative to U235 (IR) kBq U235 eq 1.98E+00 0 5.82E-06 0 9.07E-04 0
Comparative toxic unit for ecosystems (ETP-fw) CTUe 9.63E+01 0 1.85E-01 0 4.12E-01 0
Comparative toxic unit for humans (carcinogenic) (HTP-c) CTUh 7.67E-08 0 2.97E-12 0 6.28E-11 0
Comparative toxic unit for humans (noncarcinogenic) (HTP-nc) CTUh 8.61E-06 0 1.03E-10 0 6.96E-09 0
Soil quality index (SQP) SQP 4.79E+02 0 4.6E-04 0 1.53E-01 0
Disclaimer 1 – for the indicator 'Potential Human exposure efficiency relative to U235'.
This impact category deals mainly with the eventual impact of low-dose ionizing radiation on human health of the nuclear fuel cycle. It
does not consider effects due to possible nuclear accidents, occupational exposure or radioactive waste disposal in underground
facilities. Potential ionizing radiation from the soil, radon and from some construction materials is also not measured by this indicator.
Disclaimer 2 – for the indicators 'abiotic depletion potential for non-fossil resources', 'abiotic depletion potential for fossil resources',
'water (user) deprivation potential, deprivation-weighted water consumption', 'potential comparative toxic unit for ecosystems', 'potential
comparative toxic unit for humans – cancerogenic', 'Potential comparative toxic unit for humans - not cancerogenic', 'potential soil
quality index'.
The results of this environmental impact indicator shall be used with care as the uncertainties on these results are high as there is
limited experience with the indicator.
6. LCA: Interpretation
The following interpretation contains a summary of the LCA mineral ceiling tiles.
results referenced to a declared unit of 1 m² Classic Max
The comparison of the product's life cycle phases shows a C4) have a minor contribution.
clear dominance of the production phase (modules A1–A3) in
all environmental impact categories. The potential The upstream supply chain of the raw board plays a dominant
environmental impacts from transport to disposal (module C2) role in all categories.
and the End of Life of the products due to landfilling (module
7. Requisite evidence
7.1 Radioactivity and Experimental Medicine
Not applicable for these products. Certificate number: 02G15015 (5 September 2016)
Test substance: Slag Wool 'Arm SW15'
7.2 Biopersistence
The mineral wool used for the production of the panels is 7.3 VOC Emissions
biosoluble. Measuring point: China National Fiberglass Product Quality
Measuring point: Fraunhofer Institute for Toxicology Inspection & Testing Center
6 Environmental Product Declaration - Knauf Ceiling Solutions GmbH & Co. KG - Classic Max
Test report: VOC emissions test report
Test Results
Report No: 23102129
Name Value Unit
Testing periode: 8.10.2023-8.11.2023
Test basis: GB/T 25998-2020 & HJ 571-2010 TVOC after 72h 0.065 mg/(m²*h)
Formaldehyde after 52h < 0.005 mg/m³
8. References
Standards Reverberation Room Method.
ASTM E84 ASTM E1414
ASTM E84, Standard Test Method for Surface Burning ASTM E1414/E1414M-21a, Standard Test Method for Airborne
Characteristics of Building Materials. Sound Attenuation Between Rooms Sharing a Common Ceiling
Plenum.
BS 476
BS 476-6:1989+A1:2009. Fire tests on building materials and
structures. Method of test for fire propagation for products. Further References
BS 476-7:1997. Fire tests on building materials and structures.
Method of test to determine the classification of the surface AVV, German List of Wastes Ordinance
spread of flame of products. Regulation on the European Waste List. Waste Catalogue
Ordinance (German designation: Abfallverzeichnisverordnung –
DIN 18177 AVV) of 10 December 2001 (Federal Law Gazette I p. 3379),
DIN 18177:2020-12, Wet-felt factory-produced mineral panels. last amended by Article 1 of the Ordinance of 30 June 2020
(Federal Law Gazette I p. 3005).
EN 15804
DIN EN 15804:2012+A2:2019+AC:2021, Sustainability of Chemicals Prohibition Ordinance
construction works – Environmental product declarations – Chemicals Prohibition Ordinance (German designation:
Core rules for the product category of construction products. Chemikalien-Verbotsverordnung – ChemVerbotsV) of 20
January 2017 (Federal Law Gazette I p. 94; 2018 I p. 1389),
GB/T 25998 last amended by Article 300 of the Ordinance of 19 June 2020
GB/T 25998, Mineral wool decorating and acoustic ceilings. (Federal Law Gazette I p. 1328).
HJ 571-2010 China National Fiberglass Product Quality Inspection &
HJ 571-2010, Technical requirement for environmental labelling Testing Center
products – Wood-based panels and finishing products. Test report: VOC emission test
Report No: 23102129
ISO 354
DIN EN ISO 354:2003-12, Acoustics – Measurement of sound ECHA-candidate list
absorption in reverberant rooms. List of substances of very high concern (SVHC) for
authorisation (ECHA Candidate List), 25.06.2020, published
ISO 9001 under Article 59(10) of REACH. Helsinki: European Chemicals
DIN EN ISO 9001:2015-11, Quality management systems – Agency.
Requirements.
Fraunhofer Institute for Toxicology and Experimental
ISO 10848 Medicine
DIN EN ISO 10848-2:2006-08, Acoustics – Measurement of Certificate number: 02G15015 (5 September 2016); Test
airborne and impact sound transmission between adjacent substance: Slag Wool 'Arm SW15'.
rooms in test stands – Part 2: Application to lightweight
components where the connection has a minor influence. GaBi
GaBi 10, Software-System and Database for Life Cycle
ISO 14001 Engineering. DB 2022.2. Sphera, 1992–2022. Available at:
DIN EN ISO 14001:2015-11, Environmental management https://gabi.sphera.com/support/gabi/
systems – Requirements with guidance for use.
IBU 2021
ISO 14025 Institut Bauen und Umwelt e.V.: General instructions for the
DIN EN ISO 14025:2011-10, Environmental labels and EPD programme of Institut Bauen und Umwelt e.V. (IBU).
declarations – Type III environmental declarations – Principles Version 2.0, Berlin: Institut Bauen und Umwelt e.V., 2021.
and procedures. www.ibuepd.com
ISO 14044 Ordinance on Biocide Products
DIN EN ISO 14044:2006-10, Environmental management – Life Regulation (EU) No 528/2012 of the European Parliament and
cycle assessment – Requirements and guidelines. of the Council of 22 May 2012 concerning the making available
on the market and use of biocidal products.
ISO 45001
DIN ISO 45001:2018-06, Occupational health and safety Ordinance on Hazardous Substances
management systems – Requirements with guidance for use. Ordinance on Hazardous Substances, of 26 November 2010
(Federal Law Gazette I p. 1643, 1644), last amended by Article
ASTM C 423-01 148 of the Law of 29 March 2017 (Federal Law Gazette I p.
ASTM C423-01:2001-07, Standard Test Method for Sound 626).
Absorption and Sound Absorption Coefficients by the
7 Environmental Product Declaration - Knauf Ceiling Solutions GmbH & Co. KG - Classic Max
PCR Part A 31.05.2023.
Product category rules for building-related products and
services. Part A: Calculation rules for the life cycle assessment REACH
and requirements on the project report according to Regulation (EC) No 1907/2006 of the European Parliament and
EN15804+A2:2019. Version 1.3, Berlin: Institut Bauen und Council from 18 December 2006, Regulation concerning the
Umwelt e.V. (Hrsg.), 2022. Registration, Evaluation, Authorisation and Restriction of
Chemicals (REACH).
PCR: Mineral panels
Institut Bauen und Umwelt e.V. (IBU), 2023. Product Category
Rules for Building-Related Products and Services. Part B:
Requirements on the EPD for Mineral panels. Version v2,
8 Environmental Product Declaration - Knauf Ceiling Solutions GmbH & Co. KG - Classic Max
Publisher
Institut Bauen und Umwelt e.V. +49 (0)30 3087748- 0
Hegelplatz 1 info@ibu-epd.com
10117 Berlin www.ibu-epd.com
Germany
Programme holder
Institut Bauen und Umwelt e.V. +49 (0)30 3087748- 0
Hegelplatz 1 info@ibu-epd.com
10117 Berlin www.ibu-epd.com
Germany
Author of the Life Cycle Assessment
Daxner & Merl GmbH +43 676 849477826
Lindengasse 39/8 office@daxner-merl.com
1070 Wien www.daxner-merl.com
Austria
Owner of the Declaration
Knauf Ceiling Solutions GmbH & Co. KG 0049 8552 422 0
Elsenthal 15 info@knaufamf.com
94481 Grafenau www.knaufceilingsolutions.com
Germany
9 Environmental Product Declaration - Knauf Ceiling Solutions GmbH & Co. KG - Classic Max
