ENVIRONMENTAL PRODUCT DECLARATION
as per ISO 14025 and EN 15804+A2
Owner of the Declaration Gemeinschaft umweltfreundlicher Teppichboden (GUT) e.V.
Programme holder Institut Bauen und Umwelt e.V. (IBU)
Publisher Institut Bauen und Umwelt e.V. (IBU)
Declaration number EPD-GUT-20220343-CBG1-EN
Issue date 01.02.2023
Valid to 31.01.2028
Tufted wall-to-wall carpet - luxury class LC3
with a pile material made of polyamide 6
maximum surface pile weight 800 g/m2,
maximum total pile weight 1050 g/m2,
textile backing with a maximum weight of 250 g/m2
Gemeinschaft umweltfreundlicher
Teppichboden (GUT)
www.ibu-epd.com | https://epd-online.com
Umwelt Produktdeklaration Name des Herstellers – Name des Produkts
General Information
Gemeinschaft umweltfreundlicher Tufted wall-to-wall carpet - luxury
Teppichboden (GUT) e.V. class LC3, with a PA 6 pile material,
max. surface pile weight 800 g/m2,
max. total pile weight 1050 g/m2, textile
backing with a max. weight of 250 g/m2
Programme holder Owner of the declaration
IBU – Institut Bauen und Umwelt e.V. Gemeinschaft umweltfreundlicher Teppichboden e.V.
Hegelplatz 1 Schönebergstraße 2
10117 Berlin 51068 Aachen
Germany Germany
Declaration number Declared product / declared unit
EPD-GUT-20220343-CBG1-EN 1 m² tufted wall-to-wall carpet, luxury class LC3, PA 6
pile material with a textile backing.
This declaration is based on the product Scope:
category rules: This sample EPD applies to all products of the member
Floor coverings, 02/2018 companies of the Gemeinschaft umweltfreundlicher
(PCR checked and approved by the SVR) Teppichboden (GUT) e.V. that comply with the product
descriptions and are registered in the GUT/PRODIS
information system. It is only valid in conjunction with a
Issue date
valid GUT/PRODIS license of the product.
01.02.2023
The construction and production data of the registered
products are provided by the member companies of
Valid to
the GUT e.V.. The production sites are located in
31.01.2028 Belgium, Denmark, France, Germany, the Netherlands
and Switzerland.
The owner of the declaration shall be liable for the
underlying information and evidence; the IBU shall not
be liable with respect to manufacturer information, life
cycle assessment data and evidences.
The EPD was created according to the specifications
of EN 15804+A2. In the following, the standard will be
simplified as EN 15804.
Verification
The standard EN 15804 serves as the core PCR
Independent verification of the declaration and data
according to ISO 14025:2011
Dipl. Ing. Hans Peters internally x externally
(chairman of Institut Bauen und Umwelt e.V.)
Dr. Alexander Röder Angela Schindler
(Managing Director Institut Bauen und Umwelt e.V.)) (Independent verifier)
Product
Product description/Product definition Regulation (CPR) applies. The product needs a
The declaration applies to tufted wall-to-wall carpets Declaration of Performance (DoP) taking into
having a pile material of polyamide 6 and a textile consideration EN 14041:2018-05, Resilient, textile and
backing with a maximum weight of 250 g/m2. laminate floor coverings - Essential characteristics, and
The products correspond to luxury class LC3 with a the CE-marking. The DoP of the product can be found
limitation of the maximum surface pile weight of 800 on the manufacturer's technical information section.
g/m² and a maximum total pile weight of 1050 g/m2. For the application and use of the product the
Colouring and design of the use layer may be achieved respective national provisions apply.
by aqueous dyeing methods or by using solution-dyed
yarns. Application
For the placing on the market of the specific product in The use class of the specific product as defined in
the European Union/European Free Trade Association EN 1307 can be found in the Product Information
(EU/EFTA) (with the exception of Switzerland) System (PRODIS) using the PRODIS registration
Regulation (EU) No. 305/2011 Construction Product number of the product.
2 Environmental Product Declaration GUT e.V. – Tufted wall-to-wall carpet with PA6 pile material and textile backing, LC3
Polymer dispersion (solid content) 6.6 %
Technical Data Additives 3.6 %
The technical data describes a fictitious worst-case The base materials refer to the fictitious worst-case
product representing all products with the described product representing all products with the described
characteristics. characteristics.
The specific product covered by the EPD contains
Constructional data according to EN 1307 substances listed in the ECHA candidate list
Name Value Unit (08.07.2021) or other carcinogenic, mutagenic or
wall-to-wall reprotoxic (CMR) substances in categories 1A or 1B
Product Form carpet on - which are not on the candidate list exceeding 0.1
rolls percentage by mass: no
Tufted The products are registered in the GUT-PRODIS
Type of manufacture -
carpet Information System. The PRODIS system ensures the
Polyamide compliance with limitations of various chemicals and
Yarn type -
6 Volatile Organic Compound (VOC)-emissions and a
Total carpet weight max. 2800 g/m2 ban on the use of all substances that are listed as
Surface pile weight max. 800 g/m2 'Substances of Very High Concern' (SVHC) under
Textile REACH.
Secondary backing -
backing
Reference service life
The service life of textile floor coverings strongly
Performance data of the product in accordance with depends on the correct installation taking into account
the declaration of performance with respect to its the declared use classification and the adherence to
essential characteristics according to EN 14041: 2018- cleaning and maintenance instructions.
05, Resilient, textile and laminate floor coverings - A calculation of the reference service life according to
Essential characteristics. ISO 15686 is not possible.
Additional product properties in accordance with EN Alternatively, a reference service life of 10 years can
1307 can be found on the Product Information System be assumed, during which the functional and visual
PRODIS using the PRODIS registration number of the quality is guaranteed (BNB, Nutzungsdauer von
product (www.pro-dis.info) or on the manufacturer's Bauteilen). The technical service life can be
technical information section. significantly longer.
Base materials/Ancillary materials
Name Value Unit
Polyamide 6 37.5 %
Polyester 6.8 %
Polypropylene 6.8 %
Mineral Filler 33.3 %
Aluminiumhydroxide 5.4 %
LCA: Calculation rules
Declared Unit Cradle-to-gate with options, module C1-C4, module D,
and additional modules A4, A5, B1, B2.
Name Value Unit System boundaries of modules A, B, C, D:
Declared unit 1 m2 Modules C3, C4 and D are indicated separately for
Grammage 2.8 kg/m2 three end-of-life scenarios:
The declared unit refers to 1 m2 produced textile floor 1 - landfill disposal
covering. The Output of module A5 'Assembly' is 1 m2 2 - municipal waste incineration
installed textile floor covering. 3 - recovery in a cement plant
The layer thickness of the specific product covered by
the EPD can be found on the Product Information A1-A3 Production:
System PRODIS using the PRODIS registration Energy supply and production of the basic material,
number of the product (www.pro-dis.info) or on the processing of secondary material, auxiliary material,
manufacturer's technical information section. transport of the material to the manufacturing site,
emissions, waste water treatment, packaging material
The LCA results refer to the fictitious worst-case and waste processing up to the landfill disposal of
product, which covers all products of the members of residual waste (except radioactive waste). Benefits for
the GUT e.V. that correspond to the product generated electricity and steam due to the incineration
descriptions and are registered in the GUT/PRODIS of production waste are aggregated.
information system. Biogenic carbon that is stored in renewable material
(packaging paper) is taken into account as well as the
associated carbon dioxide uptake from the air from
System boundary which this biogenic carbon comes.
Type of EPD: A4 Transport:
3 Environmental Product Declaration GUT e.V. – Tufted wall-to-wall carpet with PA6 pile material and textile backing, LC3
Transport of the packed textile floor covering The floor covering is de-constructed manually and no
from factory gate to the place of installation. additional environmental impact is caused.
C2 Transport:
Transport of the carpet waste to a landfill, to the
municipal waste incineration plant (MWI) or to the
A5 Installation: waste collection facility for recycling.
Installation of the textile floor covering, processing of
installation waste and packaging waste up to the C3 Waste processing:
landfill disposal of residual waste (except radioactive C3-1: Landfill disposal needs no waste processing.
waste), the production of the amount of carpet that C3-2: Impact from waste incineration (plant with
occurs as installation waste including its transport to R1>0.6), generated electricity and steam are listed in
the place of installation. the result table as exported energy.
Generated electricity and steam due to the incineration C3-3: Collection of the carpet waste for recovery in the
of waste are listed in the result table as exported cement industry, waste processing (granulating),
energy. transport to the cement plant, emissions from the
Biogenic carbon that is stored in renewable materials incineration.
in packaging paper is released as carbon dioxide
emissions into the air at the end of life in module A5. C4 Disposal
Preparation of the floor and auxiliary materials C4-1: Impact from landfill disposal,
(adhesives, fixing agents, PET connectors) are beyond C4-2: The carpet waste leaves the system in
the system boundaries and not taken into account. module C3-2,
C4-3: The pre-processed carpet waste leaves the
B1 Use: system in module C3-3.
Indoor emissions during the use stage. After the first
year, no product-related Volatile Organic Compound D Recycling potential:
(VOC) emissions are relevant due to known VOC Calculated benefits result from materials exclusive
decay curves of the product. secondary materials (net materials).
D-A5: Benefits for generated energy due
B2 Maintenance: to incineration of packaging and installation waste
Cleaning of the textile floor covering for a period of 1 (incineration plant with R1 > 0.6),
year: D-1: Benefits for generated energy due to landfill
Vacuum cleaning – electricity supply disposal of carpet waste at the end of life,
Wet cleaning – electricity, water consumption, D-2: Benefits for generated energy due to incineration
production of the cleaning agent, waste water of carpet waste at the end-of-life (incineration plant
treatment. with R1 > 0.6),
The declared values in this module have to be D-3: Benefits for saved fossil energy and saved
multiplied by the assumed service life of the floor inorganic material due to recovery of the carpet in a
covering in the building in question. cement plant.
B3 - B5: Comparability
The modules are not relevant within the assumed Basically, a comparison or an evaluation of EPD data
reference service life of 10 years. is only possible if all the data sets to be compared
were created according to EN 15804 and the building
B6 - B7: context, respectively the product-specific
No energy and water input are required for the characteristics of performance, are taken into account.
operation of the carpet in the use stage. The modules
are not relevant and not declared. Background data are taken from the GaBi database,
2021-2. Remaining data gaps are covered by the
C1 De-construction: ecoinvent 3.7 database, 2020.
LCA: Scenarios and additional technical information
Characteristic product properties Capacity utilisation (including
55 %
Information on biogenic carbon empty runs)
Installation in the building (A5)
Name Value Unit Name Value Unit
Biogenic carbon content in Material loss 0.252 kg
accompanying packaging at factory 0.005 kg C Polyethylene packaging waste and installation waste
gate are considered to be incinerated in a municipal waste
1 kg biogenic Carbon is equivalent to 44/12 kg of CO 2 incineration plant. Cardboard packaging waste is going
to be recycled.
Preparation of the floor and auxiliaries (adhesives,
fixing agents, PET connectors etc.) are not taken into
Transport to the construction site (A4) account.
Name Value Unit
Litres of fuel (truck, EURO 0-6 Maintenance (B2)
0.0066 l/100km
mix) The values for cleaning refer to 1 m2 floor covering per
Transport distance 700 km year.
4 Environmental Product Declaration GUT e.V. – Tufted wall-to-wall carpet with PA6 pile material and textile backing, LC3
Depending on the application based on ISO 10874, the
technical service life recommended by the Reuse, recovery and/or recycling potentials (D),
manufacturer and the anticipated strain on the floor by relevant scenario information
customers, the case-specific useful life can be Recovery or recycling potentials due to the three end
established. Based on this useful life the effects of of life scenarios (module C) are indicated separately.
module B2 need to be calculated in order to obtain the
overall environmental impacts. Recycling in the cement industry (scenario 3)
The organic material of the carpet is used as an
alternative fuel in a cement kiln. It mainly substitutes
Name Value Unit for lignite (68.8 %), hard coal (23.6 %) and petrol coke
Maintenance cycle (vacuum Number (7.6 %). The inorganic material is substantially
156
cleaning) /year integrated into the cement clinker and substitutes for
Number the original material input. VDZ e.V.
Maintenance cycle (wet cleaning) 0.92
/year
Water consumption (wet cleaning) 0.0027 m3
Cleaning agent (wet cleaning) 0.055 kg
Electricity consumption 0.326 kWh
The values result from the calculation of a mixed
scenario for use in object areas and in private areas.
Maintenance cycle vacuum cleaning: 4 times per week
in object areas, 2 times per week in private areas.
Maintenance cycle wet cleaning: 3 times per 2 years in
object areas, 1 time per 3 years in private areas.
Service life
Name Value Unit
Life Span (according to
10 a
BBSR)
Corresponds to the
Declared product properties
specifications of EN -
(at the gate) and finishes
1307
An assumed quality of work,
Conforms to the
when installed in accordance
manufacturer's -
with the manufacturer’s
instructions
instructions
Use in areas
Usage conditions, e.g.
defined by the use
frequency of use, mechanical -
class according to
exposure
EN 1307
Maintenance e.g. required
According to the
frequency, type and quality
manufacturers' -
and replacement of
instructions
components
End of Life (C1-C4)
Three different end-of-life scenarios are declared and
the results are indicated separately in module C.
Each scenario is calculated as a 100 % scenario.
Scenario 1: 100 % landfill disposal
Scenario 2: 100 % municipal waste incineration (MWI)
with R1>0.6
Scenario 3: 100 % recovery in the cement industry
If combinations of these scenarios have to be
calculated this should be done according to the
following scheme:
EOL-impact = x % impact (Scenario 1)
+ y % impact (Scenario 2)
+ z % impact (Scenario 3)
with x % + y % + z % = 100 %
Name Value Unit
Collected as mixed construction
2.8 kg
waste (scenarios 1 and 2)
Collected separately (scenario 3) 2.8 kg
Landfilling (scenario 1) 2.8 kg
Energy recovery (scenario 2) 2.8 kg
Energy recovery (scenario 3) 1.716 kg
Recycling (scenario 3) 1.084 kg
5 Environmental Product Declaration GUT e.V. – Tufted wall-to-wall carpet with PA6 pile material and textile backing, LC3
LCA: Results
The modules C3/1, C4/2 and C4/3 cause no additional impact (see chapter "LCA: Calculation rules").
Module C2 represents the transport for scenarios 1, 2 and 3. The values in column D result from module A5.
DESCRIPTION OF THE SYSTEM BOUNDARY (X = INCLUDED IN LCA; ND = MODULE OR INDICATOR NOT
DECLARED; MNR = MODULE NOT RELEVANT)
BENEFITS AND
CONSTRUCTI LOADS
PRODUCT STAGE ON PROCESS USE STAGE END OF LIFE STAGE BEYOND THE
STAGE SYSTEM
BOUNDARIES
6 Environmental Product Declaration GUT e.V. – Tufted wall-to-wall carpet with PA6 pile material and textile backing, LC3
lairetam
waR
ylppus tropsnarT
gnirutcafunaM
eht
morf
tropsnarT
etis
eht
ot
etag
ylbmessA esU
ecnanetniaM
riapeR
tnemecalpeR tnemhsibrufeR
ygrene
lanoitarepO esu
retaw
lanoitarepO esu
noitcurtsnoc-eD
noitilomed tropsnarT
gnissecorp
etsaW
lasopsiD -esueR -yrevoceR -gnilcyceR laitnetop
A1 A2 A3 A4 A5 B1 B2 B3 B4 B5 B6 B7 C1 C2 C3 C4 D
X X X X X X X MNR MNR MNR ND ND X X X X X
RESULTS OF THE LCA - ENVIRONMENTAL IMPACT according to EN 15804+A2: 1 m² floor covering
Core Indicator Unit A1-A3 A4 A5 B1 B2 C1 C2 C3/2 C3/3 C4/1 D D/1 D/2 D/3
-
GWP-total [kg CO2-Eq.] 1.48E+11.71E-12.00E+00.00E+03.85E-10.00E+09.49E-34.40E+04.44E+01.99E-1-2.58E-10.00E+0 1.65E+0-3.36E-1
-
GWP-fossil [kg CO2-Eq.] 1.48E+11.68E-11.98E+00.00E+02.62E-10.00E+09.32E-34.40E+04.44E+01.99E-1-2.56E-10.00E+0 1.64E+0-3.36E-1
GWP-biogenic [kg CO2-Eq.] 5.25E-2 2.18E-3 2.30E-20.00E+02.99E-30.00E+01.21E-4 5.06E-4 9.38E-4 2.37E-8-1.31E-30.00E+0-8.34E-3-3.37E-4
GWP-luluc [kg CO2-Eq.] 3.83E-3 9.52E-4 4.45E-40.00E+01.20E-10.00E+05.29E-5 1.15E-4 2.50E-4 9.66E-5-2.82E-50.00E+0-1.79E-4-1.57E-4
2.85E- 1.02E- 2.60E- 5.68E- 3.49E- 5.60E- 2.67E- -1.73E- -1.10E- -5.60E-
ODP [kg CFC11-Eq.] 0.00E+02.08E-80.00E+0 0.00E+0
11 14 12 16 13 13 13 12 11 13
AP [mol H+-Eq.] 2.29E-2 1.02E-3 2.60E-30.00E+06.17E-40.00E+05.63E-5 4.71E-3 4.88E-3 5.88E-4-3.36E-40.00E+0-2.14E-3-1.12E-3
EP-freshwater [kg P-Eq.] 3.21E-5 5.11E-7 2.98E-60.00E+03.31E-60.00E+02.83E-8 4.39E-7 5.52E-7 3.70E-5-3.52E-70.00E+0-2.24E-6-3.74E-7
EP-marine [kg N-Eq.] 6.50E-3 4.99E-4 8.48E-40.00E+01.45E-40.00E+02.77E-5 2.35E-3 2.42E-3 1.30E-4-9.16E-50.00E+0-5.83E-4-3.60E-4
EP-terrestrial [mol N-Eq.] 6.14E-2 5.54E-3 8.51E-30.00E+01.98E-30.00E+03.08E-4 2.63E-2 2.71E-2 1.43E-3-9.79E-40.00E+0-6.24E-3-3.94E-3
POCP [kg NMVOC-Eq.]2.10E-2 9.44E-4 2.53E-3 4.18E-4 6.66E-40.00E+05.24E-5 6.00E-3 6.16E-3 4.17E-4-2.56E-40.00E+0-1.63E-3-1.09E-3
7.92E-
ADPE [kg Sb-Eq.] 2.20E-6 1.43E-8 2.01E-70.00E+01.54E-70.00E+0 1.72E-8 2.30E-8 1.38E-8-3.88E-80.00E+0-2.45E-7-3.18E-8
10
- - -
ADPF [MJ] 2.96E+22.29E+02.70E+10.00E+04.50E+00.00E+01.27E-12.13E+02.71E+02.83E+0 0.00E+0
4.36E+0 2.78E+14.69E+1
[m³ world-Eq
WDP 7.11E-1 1.53E-3 1.33E-10.00E+07.22E-20.00E+08.48E-5 5.27E-1 5.31E-1-2.11E-3-2.70E-20.00E+0-1.71E-1-5.13E-2
deprived]
GWP = Global warming potential; ODP = Depletion potential of the stratospheric ozone layer; AP = Acidification potential of land and water; EP =
Caption Eutrophication potential; POCP = Formation potential of tropospheric ozone photochemical oxidants; ADPE = Abiotic depletion potential for non-
fossil resources; ADPF = Abiotic depletion potential for fossil resources; WDP = Water (user) deprivation potential
RESULTS OF THE LCA - INDICATORS TO DESCRIBE RESOURCE USE according to EN 15804+A2: 1 m²
floor covering
Indicator Unit A1-A3 A4 A5 B1 B2 C1 C2 C3/2 C3/3 C4/1 D D/1 D/2 D/3
PERE [MJ] 2.53E+1 1.30E-1 2.35E+0 0.00E+0 2.75E+0 0.00E+0 7.20E-3 3.32E-1 4.95E-1 2.32E-1 -1.20E+0 0.00E+0 -7.60E+0-4.35E-1
PERM [MJ] 2.30E-2 0.00E+0 -2.30E-2 0.00E+0 0.00E+0 0.00E+0 0.00E+0 0.00E+0 0.00E+0 0.00E+0 0.00E+0 0.00E+0 0.00E+0 0.00E+0
PERT [MJ] 2.53E+1 1.30E-1 2.33E+0 0.00E+0 2.75E+0 0.00E+0 7.20E-3 3.32E-1 4.95E-1 2.32E-1 -1.20E+0 0.00E+0 -7.60E+0-4.35E-1
PENRE [MJ] 2.40E+2 2.29E+0 3.02E+1 0.00E+0 4.50E+0 0.00E+0 1.27E-1 5.45E+1 5.50E+1 2.83E+0 -4.36E+0 0.00E+0 -2.78E+1-4.69E+1
PENRM [MJ] 5.55E+1 0.00E+0 -3.18E+0 0.00E+0 0.00E+0 0.00E+0 0.00E+0 -5.23E+1-5.23E+1 0.00E+0 0.00E+0 0.00E+0 0.00E+0 0.00E+0
PENRT [MJ] 2.96E+2 2.29E+0 2.71E+1 0.00E+0 4.50E+0 0.00E+0 1.27E-1 2.13E+0 2.71E+0 2.83E+0 -4.36E+0 0.00E+0 -2.78E+1-4.69E+1
SM [kg] 1.04E-2 0.00E+0 9.36E-4 0.00E+0 0.00E+0 0.00E+0 0.00E+0 0.00E+0 0.00E+0 0.00E+0 0.00E+0 0.00E+0 0.00E+0 6.44E-1
RSF [MJ] 0.00E+0 0.00E+0 0.00E+0 0.00E+0 0.00E+0 0.00E+0 0.00E+0 0.00E+0 0.00E+0 0.00E+0 0.00E+0 0.00E+0 0.00E+0 0.00E+0
NRSF [MJ] 0.00E+0 0.00E+0 0.00E+0 0.00E+0 0.00E+0 0.00E+0 0.00E+0 0.00E+0 0.00E+0 0.00E+0 0.00E+0 0.00E+0 0.00E+0 0.00E+0
FW [m³] 4.60E-2 1.47E-4 5.77E-3 0.00E+0 2.52E-3 0.00E+0 8.14E-6 1.25E-2 1.26E-2 3.30E-5 -1.14E-3 0.00E+0 -7.26E-3 -4.20E-3
PERE = Use of renewable primary energy excluding renewable primary energy resources used as raw materials; PERM = Use of
renewable primary energy resources used as raw materials; PERT = Total use of renewable primary energy resources; PENRE = Use of
non-renewable primary energy excluding non-renewable primary energy resources used as raw materials; PENRM = Use of non-
Caption
renewable primary energy resources used as raw materials; PENRT = Total use of non-renewable primary energy resources; SM = Use
of secondary material; RSF = Use of renewable secondary fuels; NRSF = Use of non-renewable secondary fuels; FW = Use of net fresh
water
RESULTS OF THE LCA – WASTE CATEGORIES AND OUTPUT FLOWS according to EN 15804+A2:
1 m² floor covering
Indicator Unit A1-A3 A4 A5 B1 B2 C1 C2 C3/2 C3/3 C4/1 D D/1 D/2 D/3
HWD [kg] 3.19E-8 1.10E-11 2.91E-9 0.00E+0 2.56E-5 0.00E+0 6.08E-133.35E-103.59E-104.34E-10-5.91E-100.00E+0 -3.77E-9-1.74E-10
NHWD [kg] 2.66E-1 3.28E-4 7.36E-2 0.00E+0 5.14E-3 0.00E+0 1.82E-5 5.42E-1 5.42E-1 2.79E+0 -2.20E-3 0.00E+0 -1.40E-2 -7.25E-2
RWD [kg] 5.69E-3 2.82E-6 5.20E-4 0.00E+0 3.74E-4 0.00E+0 1.56E-7 7.22E-5 1.14E-4 3.46E-5 -3.43E-4 0.00E+0 -2.18E-3 -8.92E-5
CRU [kg] 0.00E+0 0.00E+0 0.00E+0 0.00E+0 0.00E+0 0.00E+0 0.00E+0 0.00E+0 0.00E+0 0.00E+0 0.00E+0 0.00E+0 0.00E+0 0.00E+0
MFR [kg] 2.12E-2 0.00E+0 1.39E-2 0.00E+0 0.00E+0 0.00E+0 0.00E+0 0.00E+0 6.44E-1 0.00E+0 0.00E+0 0.00E+0 0.00E+0 0.00E+0
MER [kg] 0.00E+0 0.00E+0 0.00E+0 0.00E+0 0.00E+0 0.00E+0 0.00E+0 0.00E+0 0.00E+0 0.00E+0 0.00E+0 0.00E+0 0.00E+0 0.00E+0
EEE [MJ] 0.00E+0 0.00E+0 1.15E+0 0.00E+0 0.00E+0 0.00E+0 0.00E+0 7.31E+0 0.00E+0 0.00E+0 0.00E+0 0.00E+0 0.00E+0 0.00E+0
EET [MJ] 0.00E+0 0.00E+0 2.08E+0 0.00E+0 0.00E+0 0.00E+0 0.00E+0 1.33E+1 5.23E+1 0.00E+0 0.00E+0 0.00E+0 0.00E+0 0.00E+0
HWD = Hazardous waste disposed; NHWD = Non-hazardous waste disposed; RWD = Radioactive waste disposed; CRU = Components
Caption
for re-use; MFR = Materials for recycling; MER = Materials for energy recovery; EEE = Exported electrical energy; EET = Exported
thermal energy
RESULTS OF THE LCA – additional impact categories according to EN 15804+A2-optional:
1 m² floor covering
Indicator Unit A1-A3 A4 A5 B1 B2 C1 C2 C3/2 C3/3 C4/1 D D/1 D/2 D/3
[Disease
PM 1.64E-7 5.88E-9 1.70E-8 0.00E+0 4.27E-8 0.00E+03.26E-10 1.65E-8 1.76E-8 5.65E-9 -2.79E-9 0.00E+0 -1.78E-8 -2.18E-8
Incidence]
[kBq U235-
IRP 8.79E-1 4.13E-4 8.04E-2 0.00E+0 6.58E-2 0.00E+0 2.29E-5 1.10E-2 1.81E-2 5.11E-3 -5.81E-2 0.00E+0 -3.69E-1 -9.27E-3
Eq.]
ETP-fw [CTUe] 1.30E+2 1.59E+0 1.19E+1 3.60E-3 2.03E+0 0.00E+0 8.80E-2 9.15E-1 1.25E+0 2.76E+0 -9.57E-1 0.00E+0-6.07E+0-8.13E+0
-4.40E- -2.80E- -8.55E-
HTP-c [CTUh] 4.48E-9 3.21E-114.12E-100.00E+03.90E-100.00E+01.78E-124.96E-115.73E-111.24E-10 0.00E+0
11 10 11
HTP-nc [CTUh] 1.93E-7 1.90E-9 1.78E-8 2.60E-11 6.19E-9 0.00E+01.05E-10 2.86E-9 3.24E-9 1.04E-8 -1.69E-9 0.00E+0 -1.08E-8 -4.84E-9
SQP [-] ND ND ND ND ND ND ND ND ND ND ND ND ND ND
PM = Potential incidence of disease due to PM emissions; IR = Potential Human exposure efficiency relative to U235; ETP-fw = Potential
Caption comparative Toxic Unit for ecosystems; HTP-c = Potential comparative Toxic Unit for humans (cancerogenic); HTP-nc = Potential
comparative Toxic Unit for humans (not cancerogenic); SQP = Potential soil quality index
No substantiated values can be given for the SQP indicator with the existing database.
The result figures given in module B2 refer to a period of 1 year because a reference service life is not declared.
They have to be multiplied by the assumed service life (in years) of the floor covering in the building under
consideration.
Disclaimer 1 – for the indicator “Potential Human exposure efficiency relative to U235”.
This impact category deals mainly with the eventual impact of low dose ionizingradiation on human health of the
nuclear fuel cycle. It does not consider effects due to possible nuclear accidents, occupational exposure nor due
to radioactive waste disposal in undergroundfacilities. Potential ionizing radiation from the soil, from radon and
from some construction materials is also not measured by this indicator.
Disclaimer 2 – for the indicators “abiotic depletion potential for non-fossil resources”, “abiotic depletion potential
for fossil resources”, “water (user) deprivation potential, deprivation-weighted water consumption”, “potential
comparative toxic unit for ecosystems”, “potential comparative toxic unit for humans – cancerogenic”, “Potential
comparative toxic unit for humans - not cancerogenic”, “potential soil quality index”.
The results of this environmental impact indicator shall be used with care as the uncertainties on these results are
high or as there is limited experience with the indicator.
References
EN 1307 ISO 14040
DIN EN 1307: 2014+A1:2016+A2:2018-05: Textile DIN EN ISO 14040:2006+A1:2020 Environmental
floor coverings - Classification management - Life cycle assessment - Principles and
framework
EN 13501-1
DIN EN 13501-1:2019-05: Fire classification of ISO 14044
construction products and building elements - Part 1: DIN EN ISO 14044:2006+A1:2018+A2:2020
Classification using data from reaction to fire tests Environmental management - Life cycle assessment -
Requirements and guidelines
EN 14041
DIN EN 14041: 2018-05 and DIN EN 14041: 2008-05: ISO 15686
Resilient, textile and laminate floor coverings - ISO 15686: Buildings and constructed assets -
Essential characteristics Service life planning
ISO 15686-1: 2011-05: Part 1: General principles and
EN 15804 framework
DIN EN 15804:2012+A2:2019 + AC:2021, ISO 15686-2: 2012-05: Part 2: Service life prediction
Sustainability of construction works — Environmental procedures
Product Declarations — Core rules for the product ISO 15686-7: 2017-04: Part 7: Performance
category of construction products evaluation for feedback of service life data
from practice
EN 16810 ISO 15686-8: 2008-06: Part 8: Reference service life
DIN EN 16810: 2017-08: Resilient, textile and laminate and service-life estimation
floor coverings – Environmental product declarations –
Product category rules Regulation (EU) No. 305/2011
Regulation No. 305/2011 Construction Products
ISO 10874 Regulation (CPR) of the European Council and of the
DIN EN ISO 10874: 2012+A1:2021-04: Resilient, European Parliament, April 2011
textile and laminate floor coverings - Classification
General Instructions for the IBU-EPD Program
ISO 14025 General Instructions for the EPD-Program of the
DIN EN /ISO 14025:2011-10/, Environmental labels Institut Bauen und Umwelt e.V., The Preparation of
and declarations — Type III environmental Environmental Product Declarations - EPDs, version
declarations — Principles and procedures
7 Environmental Product Declaration GUT e.V. – Tufted wall-to-wall carpet with PA6 pile material and textile backing, LC3
2.0, Institut Bauen und Umwelt e.V., Berlin, January PCR Part B
2021, www.ibu-epd.de Product Category Rules for Building-Related Products
and Services
BNB, Nutzungsdauer von Bauteilen Part B: Requirements on the EPD for floor coverings,
Bewertungssystem Nachhaltiges Bauen (BNB), V1.2, Berlin: Institut Bauen und Umwelt e.V. (IBU),
Nutzungsdauer von Bauteilen, Bundesministerium des February 2018
Inneren, für Bau und Heimat, 24.02.2017
PRODIS
ECHA candidate list Product Information System (PRODIS) of the
Candidate List of substances of very high concern European Carpet Industry, Gemeinschaft
(SVHCs) for authorisation, 08.07.2021, European umweltfreundlicher Teppichboden e.V (GUT) and
Chemicals Agency (ECHA), Helsinki, Finland European Carpet and Rug Association
(ECRA), http://www.pro-dis.info
ecoinvent
ecoinvent, Zurich, Switzerland, database version 3.7, REACH
published September 2020 Regulation (EC) No 1907/2006 of the European
Parliament and of the Council of 18 December 2006
GaBi database concerning the Registration, Evaluation, Authorisation
GaBi Software-System and Database for Life Cycle and Restriction of Chemicals (REACH), June 2017,
Engineering, thinkstep AG, Leinfelden-Echterdingen, last update: 08.07.2021
2022-1
VDZ e.V.
PCR Part A Association of German Cement Works, Ed. Environ-
Product Category Rules for Building-Related Products mental Data of the German Cement Industry 2020
and Services Part A: Calculation Rules for the Life
Cycle Assessment and Requirements on the Project
Report according to EN 15804+A2:2019, V1.2, Berlin:
Institut Bauen und Umwelt e.V. (IBU), November 2021
8 Environmental Product Declaration GUT e.V. – Tufted wall-to-wall carpet with PA6 pile material and textile backing, LC3
Publisher
Institut Bauen und Umwelt e.V. Tel +49 (0)30 3087748- 0
Hegelplatz 1 Fax +49 (0)30 3087748- 29
10117 Berlin Mail info@ibu-epd.com
Germany Web www.ibu-epd.com
Programme holder
Institut Bauen und Umwelt e.V. Tel +49 (0)30 - 3087748- 0
Hegelplatz 1 Fax +49 (0)30 – 3087748 - 29
10117 Berlin Mail info@ibu-epd.com
Germany Web www.ibu-epd.com
Author of the Life Cycle
Assessment Tel +49 (0)241 96843 410
Gemeinschaft umweltfreundlicher Fax +49 (0)241 96843 400
Teppichboden (GUT) e.V. Mail mail@gut-ev.de
Schönebergstraße 2 Web www.gut-ev.org
52068 Aachen
Germany
Owner of the Declaration
Gemeinschaft umweltfreundlicher Tel +49 (0)241 96843 410
Teppichboden (GUT) e.V. Fax +49 (0)241 96843 400
Schönebergstraße 2 Mail mail@gut-ev.de
52068 Aachen Web www.gut-ev.org
Germany
