ENVIRONMENTAL PRODUCT DECLARATION
as per ISO 14025 and EN 15804+A2
Owner of the Declaration Gemeinschaft umweltfreundlicher Teppichboden (GUT) e.V.
Publisher Institut Bauen und Umwelt e.V. (IBU)
Programme holder Institut Bauen und Umwelt e.V. (IBU)
Declaration number EPD-GUT-20220084-CBG2-EN
Issue date 21.08.2023
Valid to 20.08.2028
Tufted carpet tiles with 100% recycled PA6 pile material and
bitumen-based heavy backing, LC3
GUT e.V.
www.ibu-epd.com | https://epd-online.com
General Information
GUT e.V. Tufted carpet tiles with 100% recycled PA6 pile
material and bitumen-based heavy backing, LC3
Programme holder Owner of the declaration
IBU – Institut Bauen und Umwelt e.V. Gemeinschaft umweltfreundlicher Teppichboden (GUT) e.V.
Hegelplatz 1 Schönebergstraße 2
10117 Berlin 52068 Aachen
Germany Germany
Declaration number Declared product / declared unit
EPD-GUT-20220084-CBG2-EN 1 m² tufted carpet tiles, luxury class LC3, PA 6 pile material with 100%
recycled content, bitumen-based heavy backing.
This declaration is based on the product category rules: Scope:
Floor coverings, 01.08.2021 This sample EPD applies to all products of the member companies of the
(PCR checked and approved by the SVR) Gemeinschaft umweltfreundlicher Teppichboden (GUT) e.V. that comply
with the product descriptions and are registered in the GUT/PRODIS
information system. It is only valid in conjunction with a valid GUT/PRODIS
Issue date license of the product.
The construction and production data of the registered products are
21.08.2023
provided by the member companies of the GUT e.V.. The production sites
are located in Belgium, France, Germany, Great Britain, Ireland and The
Netherlands.
Valid to
The owner of the declaration shall be liable for the underlying information
20.08.2028 and evidence; the IBU shall not be liable with respect to manufacturer
information, life cycle assessment data and evidences.
The EPD was created according to the specifications of EN 15804+A2. In
the following, the standard will be simplified as EN 15804.
Verification
The standard EN 15804 serves as the core PCR
Independent verification of the declaration and data according to ISO
14025:2011
internally X externally
Dipl.-Ing. Hans Peters
(Chairman of Institut Bauen und Umwelt e.V.)
Florian Pronold Angela Schindler,
(Managing Director Institut Bauen und Umwelt e.V.) (Independent verifier)
1 Environmental Product Declaration - GUT e.V. - Tufted carpet tiles with 100% recycled PA6 pile material and bitumen-based heavy backing, LC3
Product
textile and laminate floor coverings - Essential characteristics.
Product description/Product definition Additional product properties in accordance with EN 1307 can
The declaration applies to tufted carpet tiles having a pile be found on the Product Information System PRODIS using the
material of polyamide 6 with 100% recycled content and a PRODIS registration number of the product (www.pro-dis.info)
bitumen-based heavy backing with a maximum weight of 3200 or on the manufacturer's technical information section.
g/m2.The total recycled content of the carpet is 20%. The
products correspond to luxury class LC3 with a limitation of the Base materials/Ancillary materials
maximum surface pile weight of 800 g/m² and a maximum total Name Value Unit
pile weight of 1050 g/m2. Colouring and design of the use layer Polyamide 6 20.2 %
may be achieved by aqueous dyeing methods or by using
Polyester 1.7 %
solution-dyed yarns. For the placing on the market of the
Polypropylene 2.0 %
specific product in the European Union/European Free Trade
Mineral Filler 48.3 %
Association (EU/EFTA) (with the exception of Switzerland)
Regulation (EU) No. 305/2011 Construction Product Regulation Aluminumhydroxide 8.2 %
(CPR) applies. The product needs a Declaration of Bitumen 14.1 %
Performance (DoP) taking into consideration EN 14041:2018- Polymer dispersion (solid content) 3.0 %
05, Resilient, textile and laminate floor coverings - Essential
Glass fiber 0.5 %
characteristics, and the CE-marking. The DoP of the product
Additives 2.0 %
can be found on the manufacturer's technical information
section. For the application and use of the product the The base materials refer to the fictitious worst-case product
respective national provisions apply. representing all products with the described characteristics.
Application
The specific product covered by the EPD contains substances
The use class of the specific product as defined in EN 1307 can listed in the ECHA candidate list (26.07.2022) or other
be found in the Product Information System (PRODIS) using carcinogenic, mutagenic or reprotoxic (CMR) substances in
the PRODIS registration number of the product. categories 1A or 1B which are not on the candidate list
exceeding 0.1 percentage by mass: no
Technical Data
The products are registered in the GUT-PRODIS Information
The technical data describes a fictitious worst-case product
System. The PRODIS system ensures the compliance with
representing all products with the described characteristics.
limitations of various chemicals and Volatile Organic Compound
Constructional data according to EN 1307 (VOC)-emissions and a ban on the use of all substances that
Name Value Unit are listed as 'Substances of Very High Concern' (SVHC) under
REACH.
Product Form Tiles -
Type of Reference service life
Tufted carpet -
manufacture The service life of textile floor coverings strongly depends on
Polyamide 6 with 100% recycled the correct installation taking into account the declared use
Yarn type -
content classification and the adherence to cleaning and maintenance
Total carpet weight max. 5200 g/m2 instructions.
A calculation of the reference service life according to ISO
Surface pile weight max. 800 g/m2
15686 is not possible. Alternatively, a reference service life of
Secondary backing Bitumen-based heavy backing - 10 years can be assumed, during which the functional and
Performance data of the product in accordance with the visual quality is guaranteed (BNB, Nutzungsdauer von
declaration of performance with respect to its essential Bauteilen). The technical service life can be significantly longer.
characteristics according to EN 14041: 2018-05, Resilient,
LCA: Calculation rules
The LCA results refer to the fictitious worst-case product, which
Declared Unit covers all products of the members of the GUT e.V. that
correspond to the product descriptions and are registered in the
Name Value Unit GUT/PRODIS information system.
Declared unit 1 m2
System boundary
Grammage 5.2 kg/m2
Type of EPD:
Layer thickness (average for LC 3) 0.01 m Cradle-to-gate with options, module C1-C4, module D, and
Gross density (average for LC 3) 525 kg/m3 additional modules A4, A5, B1, B2.
The declared unit refers to 1 m2 produced textile floor covering. System boundaries of modules A, B, C, D:
The Output of module A5 'Assembly' is 1 m2 installed textile Modules C3, C4 and D are indicated separately for three end-
floor covering. The layer thickness of the specific product of-life scenarios:
covered by the EPD can be found on the Product Information 1 - landfill disposal
System PRODIS using the PRODIS registration number of the 2 - municipal waste incineration
product (www.pro-dis.info) or on the manufacturer's technical 3 - recovery in a cement plant
information section.
A1-A3 Production:
2 Environmental Product Declaration - GUT e.V. - Tufted carpet tiles with 100% recycled PA6 pile material and bitumen-based heavy backing, LC3
Energy supply and production of the basic material, processing The floor covering is de-constructed manually and no additional
of secondary material, auxiliary material, transport of the environmental impact is caused.
material to the manufacturing site, emissions, waste water
treatment, packaging material and waste processing up to the C2 Transport:
landfill disposal of residual waste (except radioactive waste). Transport
Potential benefits for generated electricity and steam due to the of the carpet waste to a landfill, to the municipal waste
incineration of production waste are aggregated. Biogenic incineration plant (MWI) or to the waste collection facility for
carbon that is stored in renewable material (packaging paper) is recycling.
taken into account as well as the associated carbon dioxide
uptake from the air from which this biogenic carbon comes. C3 Waste processing:
C3-1: Landfill disposal needs no waste processing.
A4 Transport: C3-2: Impact from waste incineration (plant with R1 > 0.6),
Transport of the packed textile floor covering from factory gate generated electricity and steam are listed in the result table as
to the place of installation. exported energy.
C3-3:
A5 Installation: Collection of the carpet waste for recovery in the cement
Installation of the textile floor covering, processing of industry, waste processing (granulating), transport to the
installation waste and packaging waste up to the landfill cement plant, emissions from the incineration.
disposal of residual waste (except radioactive waste), the
production of the amount of carpet that occurs as installation C4 Disposal
waste including its transport to the place of installation. C4-1: Impact from landfill disposal,
Generated electricity and steam due to the incineration of C4-2: The carpet waste leaves the system in module C3-2,
waste are listed in the result table as exported energy. Biogenic C4-3: The pre-processed carpet waste leaves the system in
carbon that is stored in renewable materials in packaging paper module C3-3.
is released as carbon dioxide emissions into the air at the end
of life in module A5. Preparation D Recycling potential:
of the floor and auxiliary materials (adhesives, fixing agents, Calculated potential benefits result from materials exclusive
PET connectors) are beyond the system boundaries and not secondary materials (net materials).
taken into account. D-A5: Potential benefits for generated energy due to
incineration of packaging and installation waste (incineration
B1 Use: plant with R1 > 0.6),
Indoor emissions during the use stage. After the first year, no D-1: Potential benefits for generated energy due to landfill
product-related Volatile Organic Compound (VOC) emissions disposal of carpet waste at the end of life,
are relevant due to known VOC decay curves of the product. D-2: Potential benefits for generated energy due to incineration
of carpet waste at the end-of-life (incineration plant with R1 >
B2 Maintenance: 0.6),
Cleaning of the textile floor covering for a period of 1 year: D-3: Potential benefits for saved fossil energy and saved
Vacuum cleaning – electricity supply inorganic material due to recovery of the carpet in a cement
Wet cleaning – electricity, water consumption, production of the plant.
cleaning agent, waste water treatment.
The declared values in this module have to be multiplied by the Geographic Representativeness
assumed service life of the floor covering in the building in Land or region, in which the declared product system is
question. manufactured, used or handled at the end of the product´s
lifespan: Europe
B3 - B5:
The modules are not relevant within the assumed reference
Comparability
service life of 10 years.
Basically, a comparison or an evaluation of EPD data is only
possible if all the data sets to be compared were created
B6 - B7:
according to EN 15804 and the building context, respectively
No energy and water input are required for the operation of the
the product-specific characteristics of performance, are taken
carpet in the use stage. The modules are not relevant and not
into account. Background data are taken from the GaBi
declared.
database, 2022-2
C1 De-construction:
LCA: Scenarios and additional technical information
Transport to the construction site (A4)
Characteristic product properties of biogenic carbon
Name Value Unit
Name ValueUnit Litres of fuel (truck, EURO 0-6 mix) 0.0123 l/100km
Biogenic carbon content in accompanying kg Transport distance 700 km
0.055
packaging at factory gate C Capacity utilisation (including empty runs) 55 %
1 kg biogenic Carbon is equivalent to 44/12 kg of CO
2 Installation in the building (A5)
Name Value Unit
Material loss 0.156 kg
Polyethylene packaging waste and installation waste are
considered to be incinerated in a municipal waste incineration
3 Environmental Product Declaration - GUT e.V. - Tufted carpet tiles with 100% recycled PA6 pile material and bitumen-based heavy backing, LC3
plant. Cardboard packaging waste is going to be recycled.
End of Life (C1-C4)
Preparation of the floor and auxiliaries (adhesives, fixing
Three different end-of-life scenarios are declared and the
agents, PET connectors etc.) are not taken into account.
results are indicated separately in module C. Each scenario is
calculated as a 100 % scenario.
Maintenance (B2) Scenario 1: 100 % landfill disposal
The values for cleaning refer to 1 m2 floor covering per year. Scenario 2: 100 % municipal waste incineration (MWI)
Depending on the application based on ISO 10874, the with R1 > 0.6
technical service life recommended by the manufacturer and Scenario 3: 100 % recovery in the cement industry
the anticipated strain on the floor by customers, the case-
specific useful life can be established. Based on this useful If combinations of these scenarios have to be calculated this
life the effects of module B2 need to be calculated in order to should be done according to the following scheme:
obtain the overall environmental impacts. EOL-impact = x % impact (Scenario 1)
+ y % impact (Scenario 2)
Name Value Unit
+ z % impact (Scenario 3)
Maintenance cycle (vacuum cleaning) 156 Number /year
with x % + y % + z % = 100 %
Maintenance cycle (wet cleaning) 0.92 Number /year
Name ValueUnit
Water consumption (wet cleaning) 0.0027 m3
Collected as mixed construction waste (scenarios 1
Cleaning agent (wet cleaning) 0.055 kg and 2) 5.2 kg
Electricity consumption 0.326 kWh Collected separately (scenario 3) 5.2 kg
The values result from the calculation of a mixed scenario for Landfilling (scenario 1) 5.2 kg
use in object areas and in private areas. Maintenance cycle Energy recovery (scenario 2) 5.2 kg
vacuum cleaning: 4 times per week in object areas, 2 times per
Energy recovery (scenario 3) 2.231 kg
week in private areas. Maintenance cycle wet cleaning: 3 times
Recycling (scenario 3) 2.969 kg
per 2 years in object areas, 1 time per 3 years in private areas.
Reuse, recovery and/or recycling potentials (D), relevant
Service life scenario information
Recovery or recycling potentials due to the three end of life
Name Value Unit
scenarios (module C) are indicated separately.
Life Span (according to BBSR) 10 a
Corresponds to the Recycling in the cement industry (scenario 3):
Declared product properties (at
specifications of EN - The organic material of the carpet is used as an alternative fuel
the gate) and finishes
1307 in a cement kiln. It mainly substitutes for lignite (68.8 %), hard
An assumed quality of work, coal (23.6 %) and petrol coke (7.6 %). The inorganic material is
Conforms to the
when installed in accordance substantially integrated into the cement clinker and substitutes
manufacturer's -
with the manufacturer’s for the original material input. VDZ e.V.
instructions
instructions
Usage conditions, e.g. Use in areas defined by
frequency of use, mechanical the use class according -
exposure to EN 1307
Maintenance e.g. required According to the
frequency, type and quality and manufacturers' -
replacement of components instructions
4 Environmental Product Declaration - GUT e.V. - Tufted carpet tiles with 100% recycled PA6 pile material and bitumen-based heavy backing, LC3
LCA: Results
The modules C3/1, C4/2 and C4/3 cause no additional impact (see chapter "LCA: Calculation rules").
Module C2 represents the transport for scenarios 1, 2 and 3. The values in column D result from module A5.
DESCRIPTION OF THE SYSTEM BOUNDARY (X = INCLUDED IN LCA; ND = MODULE OR INDICATOR NOT DECLARED; MNR =
MODULE NOT RELEVANT)
Benefits and
Construction loads beyond
Product stage Use stage End of life stage
process stage the system
boundaries
la ire ta m w a Ry lp p u s tro p s n a rT g n iru tc a fu n a M e h t m o rf tro p s n a rTe tis e h t o t e ta g y lb m e s s A e s U e c n a n e tn ia M ria p e R tn e m e c a lp e R tn e m h s ib ru fe R y g re n e la n o ita re p Oe s u re ta w la n o ita re p Oe s u n o itc u rts n o c -e Dn o itilo m e d tro p s n a rT g n is s e c o rp e ts a W la s o p s iD -e s u e R-y re v o c e R-g n ilc y c e Rla itn e to p
A1 A2 A3 A4 A5 B1 B2 B3 B4 B5 B6 B7 C1 C2 C3 C4 D
X X X X X X X MNR MNR MNR MND MND X X X X X
RESULTS OF THE LCA - ENVIRONMENTAL IMPACT according to EN 15804+A2: 1 m² floor covering
Parameter Unit A1-A3 A4 A5 B1 B2 C1 C2 C3/2 C3/3 C4/1 D D/1 D/2 D/3
GWP-total kg CO 2 eq 6.28E+00 3.17E-01 5.97E-01 0 3.85E-01 0 1.77E-02 5.5E+00 5.57E+00 3.65E-01 -2.71E-02 0 -4.07E-01 -3.6E-01
GWP-fossil kg CO 2 eq 6.47E+00 3.11E-01 4E-01 0 2.62E-01 0 1.73E-02 5.5E+00 5.57E+00 3.65E-01 -2.69E-02 0 -4.05E-01 -3.6E-01
GWP-
biogenic kg CO 2 eq -1.91E-01 4.03E-03 1.96E-01 0 2.99E-03 0 2.24E-04 8.24E-04 1.62E-03 -5.99E-08 -1.34E-04 0 -1.93E-03 -2.83E-04
GWP-luluc kg CO 2 eq 7.22E-03 1.76E-03 2.83E-04 0 1.2E-01 0 9.81E-05 3.06E-04 5.57E-04 1.79E-04 -2.85E-06 0 -4.07E-05 -1.99E-04
kg CFC11
ODP 1.26E-08 1.89E-14 3.78E-10 0 2.08E-08 0 1.05E-15 4.76E-13 8.69E-13 4.95E-13 -1.74E-13 0 -2.44E-12 -4.95E-13
eq
AP mol H+ eq 1.95E-02 1.88E-03 8.16E-04 0 6.17E-04 0 1.05E-04 5.52E-03 5.84E-03 1.09E-03 -3.45E-05 0 -5E-04 -1.46E-03
EP-
kg P eq 6.7E-05 9.43E-07 2.07E-06 0 3.31E-06 0 5.25E-08 1.08E-06 1.29E-06 6.88E-05 -3.54E-08 0 -4.99E-07 -4.76E-07
freshwater
EP-marine kg N eq 6.61E-03 9.24E-04 3.09E-04 0 1.45E-04 0 5.14E-05 2.68E-03 2.82E-03 2.42E-04 -9.46E-06 0 -1.39E-04 -4.37E-04
EP-terrestrial mol N eq 6.15E-02 1.02E-02 3.08E-03 0 1.98E-03 0 5.69E-04 2.98E-02 3.13E-02 2.65E-03 -1.02E-04 0 -1.5E-03 -4.79E-03
kg
POCP NMVOC 1.73E-02 1.75E-03 7.84E-04 4.18E-04 6.66E-04 0 9.73E-05 6.87E-03 7.15E-03 7.77E-04 -2.65E-05 0 -3.92E-04 -1.29E-03
eq
ADPE kg Sb eq 1.9E-06 2.64E-08 5.88E-08 0 1.54E-07 0 1.47E-09 3.18E-08 4.28E-08 2.56E-08 -3.93E-09 0 -5.65E-08 -3.74E-08
-6.84E -3.66E
ADPF MJ 1.32E+02 4.22E+004.22E+00 0 4.5E+00 0 2.35E-01 3.7E+00 4.77E+00 5.23E+00 -4.57E-01 0
+00 +01
m3 world
WDP eq 6.26E+00 2.83E-03 2.15E-01 0 7.23E-02 0 1.57E-04 8.06E-01 8.13E-01 -3.91E-03 -2.71E-03 0 -3.81E-02 -4.93E-02
deprived
GWP = Global warming potential; ODP = Depletion potential of the stratospheric ozone layer; AP = Acidification potential of land and water; EP =
Eutrophication potential; POCP = Formation potential of tropospheric ozone photochemical oxidants; ADPE = Abiotic depletion potential for non-fossil
resources; ADPF = Abiotic depletion potential for fossil resources; WDP = Water (user) deprivation potential)
RESULTS OF THE LCA - INDICATORS TO DESCRIBE RESOURCE USE according to EN 15804+A2: 1 m² floor covering
Parameter Unit A1-A3 A4 A5 B1 B2 C1 C2 C3/2 C3/3 C4/1 D D/1 D/2 D/3
PERE MJ 5.83E+01 2.4E-01 2.03E+00 0 2.75E+00 0 1.34E-02 6.27E-01 9.29E-01 4.3E-01 -1.2E-01 0 -1.69E+00 -5.79E-01
PERM MJ 2.46E-01 0 -2.46E-01 0 0 0 0 0 0 0 0 0 0 0
PERT MJ 5.86E+01 2.4E-01 1.78E+00 0 2.75E+00 0 1.34E-02 6.27E-01 9.29E-01 4.3E-01 -1.2E-01 0 -1.69E+00 -5.79E-01
PENRE MJ 9.27E+01 4.23E+00 4.64E+00 0 4.5E+00 0 2.36E-01 4.3E+01 4.4E+01 5.23E+00 -4.57E-01 0 -6.85E+00-3.66E+01
-3.93E -3.93E
PENRM MJ 3.97E+01 0 -4.2E-01 0 0 0 0 0 0 0 0 0
+01 +01
PENRT MJ 1.32E+02 4.23E+00 4.22E+00 0 4.5E+00 0 2.36E-01 3.71E+00 4.78E+00 5.23E+00 -4.57E-01 0 -6.85E+00-3.66E+01
SM kg 1.25E+00 0 3.76E-02 0 0 0 0 0 0 0 0 0 0 1.7E+00
RSF MJ 0 0 0 0 0 0 0 0 0 0 0 0 0 0
NRSF MJ 0 0 0 0 0 0 0 0 0 0 0 0 0 0
FW m3 1.52E-01 2.71E-04 5.19E-03 0 2.52E-03 0 1.51E-05 1.91E-02 1.94E-02 6.12E-05 -1.15E-04 0 -1.62E-03 -3.54E-03
PERE = Use of renewable primary energy excluding renewable primary energy resources used as raw materials; PERM = Use of renewable primary
energy resources used as raw materials; PERT = Total use of renewable primary energy resources; PENRE = Use of non-renewable primary energy
excluding non-renewable primary energy resources used as raw materials; PENRM = Use of non-renewable primary energy resources used as raw
materials; PENRT = Total use of non-renewable primary energy resources; SM = Use of secondary material; RSF = Use of renewable secondary fuels;
NRSF = Use of non-renewable secondary fuels; FW = Use of net fresh water
RESULTS OF THE LCA – WASTE CATEGORIES AND OUTPUT FLOWS according to EN 15804+A2:
1 m² floor covering
Parameter Unit A1-A3 A4 A5 B1 B2 C1 C2 C3/2 C3/3 C4/1 D D/1 D/2 D/3
HWD kg 3.15E-03 2.03E-11 9.45E-05 0 2.56E-05 0 1.13E-12 5.56E-10 6.01E-10 8.07E-10 -6.28E-11 0 -9.6E-10 -3.36E-10
NHWD kg 7.98E-01 6.07E-04 6.95E-02 0 5.14E-03 0 3.38E-05 1.51E+00 1.51E+00 5.18E+00 -2.26E-04 0 -3.29E-03 -2.04E-01
5 Environmental Product Declaration - GUT e.V. - Tufted carpet tiles with 100% recycled PA6 pile material and bitumen-based heavy backing, LC3
RWD kg 2.82E-03 5.21E-06 8.91E-05 0 3.74E-04 0 2.9E-07 1.35E-04 2.13E-04 6.43E-05 -3.44E-05 0 -4.84E-04 -1.22E-04
CRU kg 0 0 0 0 0 0 0 0 0 0 0 0 0 0
MFR kg 2.12E-02 0 1.27E-01 0 0 0 0 0 1.7E+00 0 0 0 0 0
MER kg 0 0 0 0 0 0 0 0 0 0 0 0 0 0
EEE MJ 0 0 2.63E-01 0 0 0 0 6.55E+00 0 0 0 0 0 0
EET MJ 0 0 4.91E-01 0 0 0 0 1.24E+01 7.29E+01 0 0 0 0 0
HWD = Hazardous waste disposed; NHWD = Non-hazardous waste disposed; RWD = Radioactive waste disposed; CRU = Components for re-use;
MFR = Materials for recycling; MER = Materials for energy recovery; EEE = Exported electrical energy; EET = Exported thermal energy
RESULTS OF THE LCA – additional impact categories according to EN 15804+A2-optional:
1 m² floor covering
Parameter Unit A1-A3 A4 A5 B1 B2 C1 C2 C3/2 C3/3 C4/1 D D/1 D/2 D/3
Disease
PM 1.66E-07 1.09E-08 6.18E-09 0 4.27E-08 0 6.05E-10 2.78E-08 2.98E-08 1.05E-08 -2.86E-10 0 0 -3.94E-08
incidence
kBq U235
IR 4.15E-01 7.64E-04 1.31E-02 0 6.58E-02 0 4.26E-05 2.05E-02 3.37E-02 9.49E-03 -5.83E-03 0 0 -1.5E-02
eq
ETP-fw CTUe 6.68E+01 2.93E+00 2.16E+00 3.6E-03 2.03E+00 0 1.63E-01 1.96E+00 2.58E+00 5.12E+00 -9.61E-02 0 0 -6.86E+00
HTP-c CTUh 3.03E-09 5.93E-11 9.58E-11 0 3.9E-10 0 3.3E-12 9.28E-11 1.07E-10 2.3E-10 -4.56E-12 0 0 -1E-10
HTP-nc CTUh 1.08E-07 3.52E-09 3.56E-09 2.6E-11 6.19E-09 0 1.96E-10 6.71E-09 7.43E-09 1.93E-08 -1.75E-10 0 0 -6.52E-09
SQP SQP ND ND ND ND ND ND ND ND ND ND ND ND ND ND
PM = Potential incidence of disease due to PM emissions; IR = Potential Human exposure efficiency relative to U235; ETP-fw = Potential comparative
Toxic Unit for ecosystems; HTP-c = Potential comparative Toxic Unit for humans (cancerogenic); HTP-nc = Potential comparative Toxic Unit for humans
(not cancerogenic); SQP = Potential soil quality index
No substantiated values can be given for the SQP indicator with the existing database.
The result figures given in module B2 refer to a period of 1 year because a reference service life is not declared. They have to be
multiplied by the assumed service life (in years) of the floor covering
in the building under consideration.
Disclaimer 1 – for the indicator 'Potential Human exposure efficiency relative to U235'. This impact category deals mainly with the
eventual impact of low dose ionizing radiation on human health of the nuclear fuel cycle. It does not consider effects due to possible
nuclear accidents, occupational exposure or radioactive waste disposal in undergroundfacilities. Potential ionizing radiation from the
soil, from radon and from some construction materials is also not measured by this indicator.
Disclaimer 2 – for the indicators 'abiotic depletion potential for non-fossil resources', 'abiotic depletion potential for fossil resources',
'water (user) deprivation potential, deprivation-weighted water consumption', 'potential comparative toxic unit for ecosystems', 'potential
comparative toxic unit for humans – cancerogenic', 'Potential comparative toxic unit for humans - not cancerogenic', 'potential soil
quality index'.
The results of this environmental impact indicator shall be used with care as the uncertainties on these results are high as there is
limited experience with the indicator.
References
EN 1307 laminate floor coverings - Classification
DIN EN 1307: 2014+A1:2016+A2:2018-05: Textile floor
coverings - Classification ISO 14025
DIN EN /ISO 14025:2011-10/, Environmental labels and
EN 13501-1 declarations — Type III environmental declarations —
DIN EN 13501-1:2019-05: Fire classification of construction Principles and procedures
products and building elements - Part 1: Classification using
data from reaction to fire tests ISO 14040
DIN EN ISO 14040:2006+A1:2020 Environmental
EN 14041 management - Life cycle assessment - Principles and
DIN EN 14041: 2018-05 and DIN EN 14041: 2008-05: framework
Resilient, textile and laminate floor coverings - Essential
characteristics ISO 14044
DIN EN ISO 14044:2006+A1:2018+A2:2020 Environmental
EN 15804 management - Life cycle assessment - Requirements and
DIN EN 15804:2012+A2:2019 + AC:2021, Sustainability of guidelines
construction works —Environmental Product Declarations —
Core rules for the product category of construction products ISO 15686
ISO 15686: Buildings and constructed assets - Service life
EN 16810 planning
DIN EN 16810: 2017-08: Resilient, textile and laminate floor ISO 15686-1: 2011-05: Part 1: General principles and
coverings – Environmental product declarations – Product framework
category rules ISO 15686-2: 2012-05: Part 2: Service life prediction
procedures
ISO 10874 ISO 15686-7: 2017-04: Part 7: Performance evaluation for
DIN EN ISO 10874: 2012+A1:2021-04: Resilient, textile and feedback of service life data from practice
6 Environmental Product Declaration - GUT e.V. - Tufted carpet tiles with 100% recycled PA6 pile material and bitumen-based heavy backing, LC3
ISO 15686-8: 2008-06: Part 8: Reference service life and Engineering, Sphera Solutions Inc., Stuttgart, 2022-2
service-life estimation
PCR Part A
Regulation (EU) No. 305/2011 Product Category Rules for Building-Related Products and
Regulation No. 305/2011 Construction Products Regulation Services Part A: Calculation Rules for the
(CPR) of the European Council and of the European Life Cycle Assessment and Requirements on the Project Report
Parliament, April 2011 according to EN 15804+A2:2019, V1.2, Berlin: Institut Bauen
und Umwelt e.V. (IBU), August 2022
General Instructions for the IBU-EPD Program
General Instructions for the EPD-Program of the Institut Bauen PCR Part B
und Umwelt e.V., The Preparation of Environmental Product Product Category Rules for Building-Related Products and
Declarations - EPDs, version 2.0, Institut Bauen und Umwelt Services Part B: Requirements on the EPD for floor coverings,
e.V., Berlin, January 2021, www.ibu-epd.de V1.2, Berlin: Institut Bauen und Umwelt e.V. (IBU), September
2022
BBSR
Bundesinstitut für Bau-, Stadt- und Raumforschung (BBSR) im PRODIS
Bundesamt für Bauwesen und Raumordnung (BBR), Bonn Product Information System (PRODIS) of the European Carpet
Industry, Gemeinschaft umweltfreundlicher Teppichboden e.V
BNB, Nutzungsdauer von Bauteilen (GUT) and European Carpet and Rug Association (ECRA),
Bewertungssystem Nachhaltiges Bauen (BNB), Nutzungsdauer http://www.pro-dis.info
von Bauteilen, Bundesministerium des Inneren, für Bau und
Heimat, 24.02.2017 REACH
Regulation (EC) No 1907/2006 of the European Parliament and
ECHA candidate list of the Council of 18 December 2006 concerning the
Candidate List of substances of very high concern (SVHCs) for Registration, Evaluation, Authorisation and Restriction of
authorisation, last update 26.07.2022, European Chemicals Chemicals (REACH), June 2017
Agency (ECHA), Helsinki, Finland
VDZ e.V.
Sphera Software and database Association of German Cement Works, Ed. Environ-mental
LCA for experts Software-System and Database for Life Cycle Data of the German Cement Industry 2020
7 Environmental Product Declaration - GUT e.V. - Tufted carpet tiles with 100% recycled PA6 pile material and bitumen-based heavy backing, LC3
Publisher
Institut Bauen und Umwelt e.V. +49 (0)30 3087748- 0
Hegelplatz 1 info@ibu-epd.com
10117 Berlin www.ibu-epd.com
Germany
Programme holder
Institut Bauen und Umwelt e.V. +49 (0)30 3087748- 0
Hegelplatz 1 info@ibu-epd.com
10117 Berlin www.ibu-epd.com
Germany
Author of the Life Cycle Assessment
Gemeinschaft umweltfreundlicher Teppichboden +49 (0)241 96843 410
(GUT) e.V. mail@gut-ev.de
Schönebergstraße 2 www.gut-ev.org
52068 Aachen
Germany
Owner of the Declaration
Gemeinschaft umweltfreundlicher Teppichboden +49 (0)241 96843 410
(GUT) e.V. mail@gut-ev.de
Schönebergstraße 2 www.gut-ev.org
52068 Aachen
Germany
8 Environmental Product Declaration - GUT e.V. - Tufted carpet tiles with 100% recycled PA6 pile material and bitumen-based heavy backing, LC3
