ENVIRONMENTAL
as per ISO 14025 and EN 15804+A2
Owner of the Declaration Interface®
Programme holder Institut Bauen und Umwelt e.V. (IBU)
Publisher Institut Bauen und Umwelt e.V. (IBU)
Declaration number EPD-INT-20220235-CBB1-EN
Issue date 17.02.2023
Valid to 16.02.2028
Modular carpet tiles with CQuestBio Sone+ acoustic
backing
pile material: solution-dyed polyamide 6.6 yarn 75% recycled
with a maximum total pile weight of 1000 g/m2
Interface®
www.ibu-epd.com | https://epd-online.com
Umwelt Produktdeklaration Name des Herstellers – Name des Produkts
General Information
Interface® Modular carpet tiles with CQuestBio
Sone+ acoustic backing
pile material: solution-dyed polyamide
6.6 yarn 75% recycled with a maximum
total pile weight of 1000 g/m2
Programme holder Owner of the declaration
IBU – Institut Bauen und Umwelt e.V. Interface Europe Manufacturing BV
Hegelplatz 1 Industrielaan 15
10117 Berlin 3925 ZG Scherpenzeel
Germany The Netherlands
Declaration number Declared product / declared unit
EPD-INT-20220235-CBB1-EN 1 m² tufted modular carpet tiles with Sone+ acoustic
felt covered CQuest Bio (CQB) heavy backing and a
pile material of PA 6.6 with 75% recycled content
This declaration is based on the product Scope:
category rules: The manufacturer declaration applies to tufted carpet
Floor coverings, 02/2018 tiles with a Sone+ polyester felt covered CQuest Bio
(PCR checked and approved by the SVR) backing, a pile material of 75% recycled PA 6.6 with a
maximum total pile weight of 1000 g/m2. The products
are tufted in Craigavon, Ireland and back coated in
Issue date
Scherpenzeel, Netherlands.
17.02.2023
LCA results for products with a maximum total pile
weight of 570 g/m2 can be taken from the
Valid to
corresponding tables of the annexe. Specific data for
16.02.2028 every product within the declared group of products in
relation to its total pile weight can be calculated by
using equation 1 given in the annexe (see annexe
chapter: 'General Information on the annexe'). The
declaration is only valid in conjunction with a valid
GUT-PRODIS license of the product.
The owner of the declaration shall be liable for the
underlying information and evidence; the IBU shall not
be liable with respect to manufacturer information, life
cycle assessment data and evidences.
The EPD was created according to the specifications
of EN 15804+A2. In the following, the standard will be
simplified as EN 15804.
Verification
The standard EN 15804 serves as the core PCR
Independent verification of the declaration and data
according to ISO 14025:2011
Dipl. Ing. Hans Peters internally x externally
(chairman of Institut Bauen und Umwelt e.V.)
Dr. Alexander Röder Prof. Dr. Birgit Grahl
(Managing Director Institut Bauen und Umwelt e.V.)) (Independent verifier)
Product
Product description/Product definition a recycled filler, glass-fleece reinforcement and
The declaration applies to tufted carpet tiles having a polyester covering fleece.
surface pile of 75% recycled solution dyed polyamide For the placing on the market of the specific product in
6.6 with a maximum total pile weight of 1000 g/m2. The the European Union/European Free Trade Association
backing of the carpet consists of a CQuest Bio backing (EU/EFTA) (with the exception of Switzerland)
covered by a Sone+ acoustic felt. The total recycled Regulation (EU) No. 305/2011 Construction Product
content of the carpet is 77%. Regulation (CPR) applies. The product needs a
CQuest Bio backing system Sone+: Backing Declaration of Performance (DoP) taking into
compound based on renewable wood resin, containing
2 Environmental Product Declaration Interface – Tufted tiles, 75% rec. PA 6.6 with a maximum total pile weight of 1000
g/m2 , CQuest Bio Sone+ backing
consideration EN 14041:2018-05, Resilient, textile and
laminate floor coverings - Essential characteristics, and Base materials/Ancillary materials
the CE-marking. The DoP of the product can be found
on the manufacturer's technical information section. Name Value Unit
For the application and use of the product the Polyamide 6.6 20.4 %
respective national provisions apply. Polyester 20.8 %
Limestone 41.1 %
Application Aluminiumhydroxide 4.7 %
The use class of the specific product as defined in Ethylene vinyl acetate (EVA) 5.3 %
EN 1307 can be found in the Product Information Wood resin 5.7 %
System (PRODIS) using the PRODIS registration Glass fiber 0.4 %
number of the product.
Additives 1.6 %
The specific product covered by the EPD contains
Technical Data
substances listed in the ECHA candidate list
The performance data listed in the Declaration of
(08.07.2021) exceeding 0.1 percentage by mass: no
Performance (DoP) apply.
This product contains other CMR substances in
categories 1A or 1B which are not on the candidate list
Constructional data according to EN 1307
exceeding 0.1 percentage by mass: no
Name Value Unit
Biocide products were added to this construction
Modular carpet tiles, 50 cm
Product Form - product or it has been treated with biocide products
x 50 cm
(this then concerns a treated product as defined by the
Type of manufacture Tufted carpet -
(EU) Ordinance on Biocide Products No. 528/2012): no
Polyamide 6.6 from 75%
Yarn type - Aluminium hydroxide is used as fire retardant.
recycled material
Total carpet weight 4897 g/m2 Reference service life
CQuest Bio backing with The service life of textile floor coverings strongly
Secondary backing acoustic textile bottom - depends on the correct installation taking into account
Sone+ the declared use classification and the adherence to
cleaning and maintenance instructions.
A calculation of the reference service life according to
Performance data of the product in accordance with ISO 15686 is not possible.
the declaration of performance with respect to its Alternatively, a reference service life of 15 years can
essential characteristics according to EN 14041: 2018- be assumed, during which the functional and visual
05, Resilient, textile and laminate floor coverings - quality is guaranteed (In accordance with the warranty
Essential characteristics. of the manufacturer). The technical service life can be
Additional product properties in accordance with EN significantly longer.
1307 can be found on the Product Information System
PRODIS using the PRODIS registration number of the
product (www.pro-dis.info) or on the manufacturer's
technical information section.
LCA: Calculation rules
Declared Unit System boundary
Type of EPD: Cradle-to-gate with options
The indicated values refer to a virtual reference System boundaries of modules A, B, C, D:
product with the max. total pile weight and the max. Modules C3, C4 and D are indicated separately for
total weight. three end-of-life scenarios:
Name Value Unit 1 - landfill disposal
Declared unit 1 m2 2 - municipal waste incineration
Grammage (declared virtual product) 4.897 kg/m2 3 - recovery in a cement plant
Total thickness (heaviest real product) 10.8 mm
Gross density (heaviest real product) 422 kg/m3 A1-A3 Production:
The declared unit refers to 1 m2 produced textile floor Energy supply and production of the basic material,
covering. The output of module A5 'Assembly' is 1 m2 processing of secondary material, auxiliary material,
installed textile floor covering. transport of the material to the manufacturing site,
As the thickness of a virtual product cannot be emissions, waste water treatment, packaging material
calculated due to the fact that the total thickness does and waste processing up to the landfill disposal of
not depend on the total weight, the declared total residual waste (except radioactive waste). Benefits for
thickness and gross density refer to the heaviest real generated electricity and steam due to the incineration
product. of production waste are aggregated.
The layer thickness of the specific product covered by Biogenic carbon that is stored in renewable material
the EPD can be found on the Product Information (wood resin, renewable additives,packaging paper) is
System PRODIS using the PRODIS registration taken into account as well as the associated carbon
number of the product (www.pro-dis.info) or on the dioxide uptake from the air from which this biogenic
manufacturer's technical information section. carbon comes.
A4 Transport:
3 Environmental Product Declaration Interface – Tufted tiles, 75% rec. PA 6.6 with a maximum total pile weight of 1000
g/m2 , CQuest Bio Sone+ backing
Transport of the packed textile floor covering
from factory gate to the place of installation. C2 Transport:
Transport of the carpet waste to a landfill, to the
A5 Installation: municipal waste incineration plant (MWI) or to the
Installation of the textile floor covering, processing of waste collection facility for recycling.
installation waste and packaging waste up to the
landfill disposal of residual waste (except radioactive C3 Waste processing:
waste), the production of the amount of carpet that C3-1: Landfill disposal needs no waste processing.
occurs as installation waste including its transport to C3-2: Impact from waste incineration (plant with R1 >
the place of installation. 0.6), generated electricity and steam are listed in the
Generated electricity and steam due to the incineration result table as exported energy.
of waste are listed in the result table as exported C3-3: Collection of the carpet waste for recovery in the
energy. cement industry, waste processing (granulating),
Biogenic carbon that is stored in renewable materials transport to the cement plant, emissions from the
in installation waste and packaging paper is released incineration.
as carbon dioxide emissions into the air at the end of
life in module A5. C4 Disposal
Preparation of the floor and auxiliary materials C4-1: Impact from landfill disposal,
(adhesives, fixing agents, PET connectors) are beyond C4-2: The carpet waste leaves the system in module
the system boundaries and not taken into account. C3-2,
C4-3: The pre-processed carpet waste leaves the
B1 Use: system in module C3-3.
Indoor emissions during the use stage. After the first
year, no product-related Volatile Organic Compound D Recycling potential:
(VOC) emissions are relevant due to known VOC Calculated benefits result from materials exclusive
decay curves of the product. secondary materials (net materials).
D-A5: Benefits for generated energy due
B2 Maintenance: to incineration of packaging and installation waste
Cleaning of the textile floor covering for a period of 1 (incineration plant with R1 > 0.6),
year: D-1: Assuming that the chemically bound renewable
Vacuum cleaning – electricity supply materials in a landfill gas do not release landfill gas
Wet cleaning – electricity, water consumption, within 100 years, no benefits due to landfill dosposal of
production of the cleaning agent, waste water carpet waste at the end-of-life are taken into account,
treatment D-2: Benefits for generated energy due to incineration
The declared values in this module have to be of carpet waste at the end-of-life (incineration plant
multiplied by the assumed service life of the floor with R1 > 0.6),
covering in the building in question. D-3: Benefits for saved fossil energy and saved
inorganic material due to recovery of the carpet in a
B3 - B5: cement plant.
The modules are not relevant within the assumed
reference service life of 15 years. Comparability
Basically, a comparison or an evaluation of EPD data
B6 - B7: is only possible if all the data sets to be compared
No energy and water input are required for the were created according to EN 15804 and the building
operation of the carpet in the use stage. The modules context, respectively the product-specific
do not cause any environmental impact. characteristics of performance, are taken into account.
C1 De-construction: Background data are taken from the GaBi database,
The floor covering is de-constructed manually and no 2022-1. Remaining data gaps are covered by the
additional environmental impact is caused. ecoinvent 3.7 database, 2020.
LCA: Scenarios and additional technical information
Characteristic product properties
Information on biogenic Carbon Transport to the construction site (A4)
Name Value Unit
Litres of fuel (truck, EURO 0-6
0.012 l/100km
Name Value Unit mix)
Biogenic carbon content in Transport distance 700 km
0.26 kg C
product at factory gate Capacity utilisation (including
55 %
Biogenic carbon content in empty runs)
accompanying packaging at 0.05 kg C
factory gate Installation in the building (A5)
1 kg biogenic Carbon is equivalent to 44/12 kg of CO 2 Name Value Unit
Material loss 0.147 kg
Polyethylene packaging waste and installation waste
are considered to be incinerated in a municipal waste
incineration plant. Cardboard packaging waste is going
to be recycled.
Preparation of the floor and auxiliaries (adhesives,
4 Environmental Product Declaration Interface – Tufted tiles, 75% rec. PA 6.6 with a maximum total pile weight of 1000
g/m2 , CQuest Bio Sone+ backing
fixing agents, PET connectors etc.) are not taken into Energy recovery (scenario 3) 2.639 kg
account. Recycling (scenario 3) 2.258 kg
Maintenance (B2) Reuse, recovery and/or recycling potentials (D),
The values for cleaning refer to 1 m2 floor covering per relevant scenario information
year. Recovery or recycling potentials due to the three end-
Depending on the application based on ISO 10874, the of-life scenarios (module C) are indicated separately.
technical service life recommended by the
manufacturer and the anticipated strain on the floor by Recycling in the cement industry (scenario 3)
customers, the case-specific useful life can be The organic material of the carpet is used as an
established. Based on this useful life the effects of alternative fuel in a cement kiln. It mainly substitutes
module B2 need to be calculated in order to obtain the for lignite (68.8%), hard coal (23.6%) and petrol coke
overall environmental impacts. (7.6%). The inorganic material is substantially
integrated into the cement clinker and substitutes for
original material input. VDZ e.V.
Name Value Unit
Number
Maintenance cycle (vacuum cleaning) 208
/year
Number
Maintenance cycle (wet cleaning) 1,5
/year
Water consumption (wet cleaning) 0.004 m3
Cleaning agent (wet cleaning) 0.09 kg
Electricity consumption 0.314 kWh
For further information on cleaning and maintenance
see www.interface.com
Service life
Name Value Unit
Life Span (according to
15 a
manufacturer's warranty)
Corresponds to
Declared product properties (at the
-
the gate) and finishes specifications of
EN 1307
An assumed quality of work, when Conforms to the
installed in accordance with the manufacturer's -
manufacturer’s instructions instructions
Use in areas
defined by the
Usage conditions, e.g. frequency
use class -
of use, mechanical exposure
according to EN
1307
Maintenance e.g. required According to the
frequency, type and quality and manufacturers -
replacement of components instructions
End of Life (C1-C4)
Three different end-of-life scenarios are declared and
the results are indicated separately in module C.
Each scenario is calculated as a 100% scenario.
Scenario 1: 100 % landfill disposal
Scenario 2: 100 % municipal waste incineration (MWI)
with R1 > 0.6
Scenario 3: 100 % recovery in the cement industry
If combinations of these scenarios have to be
calculated this should be done according to the
following scheme:
EOL-impact = x % impact (Scenario 1)
+ y % impact (Scenario 2)
+ z % impact (Scenario 3)
with x % + y % + z % = 100 %
Name Value Unit
Collected as mixed construction
4.897 kg
waste (scenario 1 and 2)
Collected separately (scenario 3) 4.897 kg
Landfilling (scenario 1) 4.897 kg
Energy recovery (scenario 2) 4.897 kg
5 Environmental Product Declaration Interface – Tufted tiles, 75% rec. PA 6.6 with a maximum total pile weight of 1000
g/m2 , CQuest Bio Sone+ backing
LCA: Results
The LCA results refer to all declared products with a maximum total pile weight of 1000 g/m2. LCA results for
products with a maximum total pile weight of 570 g/m2 can be taken from the corresponding tables of the annexe.
Results for specific products with any other total pile weight can be calculated by using equation 1 given in the
annexe (see annexe chapter: 'General Information on the annexe'). The declared result figures in module B2 have
to be multiplied by the assumed service life (in years) of the floor covering in the building under consideration.
Information on non-relevant modules: Modules B3 - B7 are not relevant during the service life of the carpet.
Modules C1, C3/1, C4/2 and C4/3 cause no additional impact (see chapter "LCA: Calculation rules" in this
document). All these modules are declared and marked as 'modules not relevant/declared'. Module C2 represents
the transport for scenarios 1, 2 and 3. Column D represents benefits from module A5 assembly.
DESCRIPTION OF THE SYSTEM BOUNDARY (X = INCLUDED IN LCA; ND = MODULE OR INDICATOR NOT
DECLARED; MNR = MODULE NOT RELEVANT)
BENEFITS AND
CONSTRUCTI LOADS
PRODUCT STAGE ON PROCESS USE STAGE END OF LIFE STAGE BEYOND THE
STAGE SYSTEM
BOUNDARIES
6 Environmental Product Declaration Interface – Tufted tiles, 75% rec. PA 6.6 with a maximum total pile weight of 1000
g/m2 , CQuest Bio Sone+ backing
lairetam
waR
ylppus tropsnarT
gnirutcafunaM
eht
morf
tropsnarT
etis
eht
ot
etag
ylbmessA esU
ecnanetniaM
riapeR
tnemecalpeR tnemhsibrufeR
ygrene
lanoitarepO esu
retaw
lanoitarepO esu
noitcurtsnoc-eD
noitilomed tropsnarT
gnissecorp
etsaW
lasopsiD -esueR -yrevoceR -gnilcyceR laitnetop
A1 A2 A3 A4 A5 B1 B2 B3 B4 B5 B6 B7 C1 C2 C3 C4 D
X X X X X X X MNR MNR MNR ND ND X X X X X
RESULTS OF THE LCA - ENVIRONMENTAL IMPACT according to EN 15804+A2: 1 m² floor covering
Core Indicator Unit A1-A3 A4 A5 B1 B2 C1 C2 C3/2 C3/3 C4/1 D D/1 D/2 D/3
GWP-total [kg CO2-Eq.] 6.72E+02.99E-1 4.88E-10.00E+04.16E-10.00E+01.66E-26.40E+06.47E+01.29E+0-2.77E-20.00E+0-4.69E-1-2.23E-1
GWP-fossil [kg CO2-Eq.] 7.73E+02.93E-1 4.62E-10.00E+02.15E-10.00E+01.63E-25.45E+05.52E+03.43E-1-2.76E-20.00E+0-4.67E-1-2.22E-1
-
GWP-biogenic [kg CO2-Eq.] 1.02E+03.79E-3 2.51E-20.00E+04.16E-30.00E+02.11E-4 9.49E-1 9.50E-1 9.48E-1-1.41E-40.00E+0-2.36E-3-3.79E-4
GWP-luluc [kg CO2-Eq.] 5.50E-3 1.66E-3 2.26E-40.00E+01.96E-10.00E+09.24E-5 2.35E-4 4.71E-4 1.69E-4-3.02E-60.00E+0-5.07E-5-1.08E-4
1.78E- 3.52E- 9.93E- 5.00E- 8.70E- 4.66E- -1.86E- -3.11E- -2.80E-
ODP [kg CFC11-Eq.] 1.17E-8 0.00E+03.42E-80.00E+0 0.00E+0
14 10 16 13 13 13 13 12 13
AP [mol H+-Eq.] 2.05E-2 1.77E-3 8.27E-40.00E+08.32E-40.00E+09.87E-5 5.12E-3 5.42E-3 1.03E-3-3.62E-50.00E+0-6.09E-4-8.55E-4
EP-freshwater [kg P-Eq.] 1.06E-4 8.89E-7 3.25E-60.00E+05.19E-60.00E+04.95E-8 8.49E-7 1.05E-6 6.48E-5-3.78E-80.00E+0-6.33E-7-2.39E-7
EP-marine [kg N-Eq.] 6.53E-3 8.70E-4 2.99E-40.00E+01.97E-40.00E+04.84E-5 2.48E-3 2.61E-3 2.28E-4-9.83E-60.00E+0-1.66E-4-2.56E-4
EP-terrestrial [mol N-Eq.] 7.00E-2 9.63E-3 3.26E-30.00E+02.83E-30.00E+05.36E-4 2.78E-2 2.93E-2 2.50E-3-1.05E-40.00E+0-1.78E-3-2.81E-3
POCP [kg NMVOC-Eq.]1.84E-2 1.65E-3 7.97E-4 4.18E-4 9.83E-40.00E+09.16E-5 6.37E-3 6.63E-3 7.32E-4-2.75E-50.00E+0-4.64E-4-7.65E-4
ADPE [kg Sb-Eq.] 3.04E-6 2.49E-8 9.28E-80.00E+02.30E-70.00E+01.39E-9 2.79E-8 3.82E-8 2.41E-8-4.15E-90.00E+0-6.97E-8-2.14E-8
- -
ADPF [MJ] 1.35E+23.98E+04.28E+00.00E+05.90E+00.00E+02.22E-13.28E+04.29E+04.93E+0-4.69E-10.00E+0
7.93E+02.53E+1
[m³ world-Eq
WDP 1.31E+12.66E-3 4.21E-10.00E+09.99E-20.00E+01.48E-4 8.08E-1 8.14E-1-3.68E-3-2.89E-30.00E+0-4.85E-2-3.20E-2
deprived]
GWP = Global warming potential; ODP = Depletion potential of the stratospheric ozone layer; AP = Acidification potential of land and water; EP =
Caption Eutrophication potential; POCP = Formation potential of tropospheric ozone photochemical oxidants; ADPE = Abiotic depletion potential for non-
fossil resources; ADPF = Abiotic depletion potential for fossil resources; WDP = Water (user) deprivation potential
RESULTS OF THE LCA - INDICATORS TO DESCRIBE RESOURCE USE according to EN 15804+A2: 1 m²
floor covering
Indicator Unit A1-A3 A4 A5 B1 B2 C1 C2 C3/2 C3/3 C4/1 D D/1 D/2 D/3
PERE [MJ] 4.31E+1 2.26E-1 1.99E+0 0.00E+0 3.69E+0 0.00E+0 1.26E-2 1.40E+1 1.43E+1 4.05E-1 -1.28E-1 0.00E+0 -2.15E+0-3.19E-1
PERM [MJ] 1.37E+1 0.00E+0 -2.60E-1 0.00E+0 0.00E+0 0.00E+0 0.00E+0 -1.34E+1-1.34E+1 0.00E+0 0.00E+0 0.00E+0 0.00E+0 0.00E+0
PERT [MJ] 5.68E+1 2.26E-1 1.73E+0 0.00E+0 3.69E+0 0.00E+0 1.26E-2 5.63E-1 8.48E-1 4.05E-1 -1.28E-1 0.00E+0 -2.15E+0-3.19E-1
PENRE [MJ] 1.22E+2 3.99E+0 4.72E+0 0.00E+0 5.90E+0 0.00E+0 2.22E-1 1.74E+1 1.84E+1 4.93E+0 -4.69E-1 0.00E+0 -7.93E+0-2.53E+1
PENRM [MJ] 1.45E+1 0.00E+0 -3.96E-1 0.00E+0 0.00E+0 0.00E+0 0.00E+0 -1.41E+1-1.41E+1 0.00E+0 0.00E+0 0.00E+0 0.00E+0 0.00E+0
PENRT [MJ] 1.36E+2 3.99E+0 4.32E+0 0.00E+0 5.90E+0 0.00E+0 2.22E-1 3.28E+0 4.29E+0 4.93E+0 -4.69E-1 0.00E+0 -7.93E+0-2.53E+1
SM [kg] 3.95E+0 0.00E+0 1.19E-1 0.00E+0 0.00E+0 0.00E+0 0.00E+0 0.00E+0 0.00E+0 0.00E+0 0.00E+0 0.00E+0 0.00E+0 1.70E-1
RSF [MJ] 0.00E+0 0.00E+0 0.00E+0 0.00E+0 0.00E+0 0.00E+0 0.00E+0 0.00E+0 0.00E+0 0.00E+0 0.00E+0 0.00E+0 0.00E+0 0.00E+0
NRSF [MJ] 0.00E+0 0.00E+0 0.00E+0 0.00E+0 0.00E+0 0.00E+0 0.00E+0 0.00E+0 0.00E+0 0.00E+0 0.00E+0 0.00E+0 0.00E+0 0.00E+0
FW [m³] 3.29E-1 2.56E-4 1.05E-2 0.00E+0 3.34E-3 0.00E+0 1.42E-5 1.91E-2 1.94E-2 5.77E-5 -1.23E-4 0.00E+0 -2.05E-3 -2.38E-3
PERE = Use of renewable primary energy excluding renewable primary energy resources used as raw materials; PERM = Use of
renewable primary energy resources used as raw materials; PERT = Total use of renewable primary energy resources; PENRE = Use of
non-renewable primary energy excluding non-renewable primary energy resources used as raw materials; PENRM = Use of non-
Caption
renewable primary energy resources used as raw materials; PENRT = Total use of non-renewable primary energy resources; SM = Use
of secondary material; RSF = Use of renewable secondary fuels; NRSF = Use of non-renewable secondary fuels; FW = Use of net fresh
water
RESULTS OF THE LCA – WASTE CATEGORIES AND OUTPUT FLOWS according to EN 15804+A2:
1 m² floor covering
Indicator Unit A1-A3 A4 A5 B1 B2 C1 C2 C3/2 C3/3 C4/1 D D/1 D/2 D/3
HWD [kg] 2.00E-7 1.91E-11 6.02E-9 0.00E+0 4.19E-5 0.00E+0 1.06E-124.84E-105.26E-107.60E-10-6.36E-110.00E+0 -1.08E-9-1.86E-10
NHWD [kg] 3.49E-1 5.72E-4 4.50E-2 0.00E+0 7.30E-3 0.00E+0 3.18E-5 1.15E+0 1.15E+0 4.88E+0 -2.37E-4 0.00E+0 -3.98E-3 -1.09E-1
RWD [kg] 7.14E-3 4.91E-6 2.18E-4 0.00E+0 3.76E-4 0.00E+0 2.73E-7 1.24E-4 1.98E-4 6.05E-5 -3.68E-5 0.00E+0 -6.16E-4 -7.03E-5
CRU [kg] 0.00E+0 0.00E+0 0.00E+0 0.00E+0 0.00E+0 0.00E+0 0.00E+0 0.00E+0 0.00E+0 0.00E+0 0.00E+0 0.00E+0 0.00E+0 0.00E+0
MFR [kg] 0.00E+0 0.00E+0 1.21E-1 0.00E+0 0.00E+0 0.00E+0 0.00E+0 0.00E+0 1.29E+0 0.00E+0 0.00E+0 0.00E+0 0.00E+0 0.00E+0
MER [kg] 0.00E+0 0.00E+0 0.00E+0 0.00E+0 0.00E+0 0.00E+0 0.00E+0 0.00E+0 0.00E+0 0.00E+0 0.00E+0 0.00E+0 0.00E+0 0.00E+0
EEE [MJ] 0.00E+0 0.00E+0 3.07E-1 0.00E+0 0.00E+0 0.00E+0 0.00E+0 8.18E+0 0.00E+0 0.00E+0 0.00E+0 0.00E+0 0.00E+0 0.00E+0
EET [MJ] 0.00E+0 0.00E+0 5.64E-1 0.00E+0 0.00E+0 0.00E+0 0.00E+0 1.51E+1 7.41E+1 0.00E+0 0.00E+0 0.00E+0 0.00E+0 0.00E+0
HWD = Hazardous waste disposed; NHWD = Non-hazardous waste disposed; RWD = Radioactive waste disposed; CRU = Components
Caption for re-use; MFR = Materials for recycling; MER = Materials for energy recovery; EEE = Exported electrical energy; EET = Exported
thermal energy
RESULTS OF THE LCA – additional impact categories according to EN 15804+A2-optional:
1 m² floor covering
Indicator Unit A1-A3 A4 A5 B1 B2 C1 C2 C3/2 C3/3 C4/1 D D/1 D/2 D/3
[Disease -3.00E-
PM 1.82E-7 1.02E-8 6.51E-9 0.00E+0 6.84E-8 0.00E+05.70E-10 2.35E-8 2.54E-8 9.89E-9 0.00E+0 0.00E+0 -1.19E-8
Incidence] 10
[kBq U235-
IRP 1.12E+0 7.20E-4 3.42E-2 0.00E+0 6.78E-2 0.00E+0 4.01E-5 1.90E-2 3.15E-2 8.93E-3 -6.23E-3 0.00E+0 0.00E+0 -8.42E-3
Eq.]
ETP-fw [CTUe] 1.18E+2 2.76E+0 3.68E+0 3.60E-3 2.69E+0 0.00E+0 1.54E-1 1.65E+0 2.23E+0 4.82E+0 -1.03E-1 0.00E+0 0.00E+0-4.60E+0
-4.73E- -6.03E-
HTP-c [CTUh] 2.08E-9 5.58E-116.68E-110.00E+06.21E-100.00E+03.11E-128.16E-119.51E-112.16E-10 0.00E+0 0.00E+0
12 11
-1.82E-
HTP-nc [CTUh] 9.29E-8 3.31E-9 3.06E-9 2.60E-11 9.46E-9 0.00E+01.84E-10 5.38E-9 6.05E-9 1.81E-8 0.00E+0 0.00E+0 -3.76E-9
10
SQP [-] ND ND ND ND ND 0.00E+0 6.11E-2 6.49E-1 9.33E-1 2.84E-1 ND ND ND ND
PM = Potential incidence of disease due to PM emissions; IR = Potential Human exposure efficiency relative to U235; ETP-fw = Potential
Caption comparative Toxic Unit for ecosystems; HTP-c = Potential comparative Toxic Unit for humans (cancerogenic); HTP-nc = Potential
comparative Toxic Unit for humans (not cancerogenic); SQP = Potential soil quality index
No substantiated values can be given for the SQP indicator with the existing database.
The result figures given in module B2 refer to a period of 1 year because a reference service life is not declared.
They have to be multiplied by the assumed service life (in years) of the floor covering in the building under
consideration.
Disclaimer 1 – for the indicator “Potential Human exposure efficiency relative to U235”.
This impact category deals mainly with the eventual impact of low dose ionizingradiation on human health of the
nuclear fuel cycle. It does not consider effects due to possible nuclear accidents, occupational exposure nor due
to radioactive waste disposal in undergroundfacilities. Potential ionizing radiation from the soil, from radon and
from some construction materials is also not measured by this indicator.
Disclaimer 2 – for the indicators “abiotic depletion potential for non-fossil resources”, “abiotic depletion potential
for fossil resources”, “water (user) deprivation potential, deprivation-weighted water consumption”, “potential
comparative toxic unit for ecosystems”, “potential comparative toxic unit for humans – cancerogenic”, “Potential
comparative toxic unit for humans - not cancerogenic”, “potential soil quality index”.
The results of this environmental impact indicator shall be used with care as the uncertainties on these results are
high or as there is limited experienced with the indicator.
References
EN 1307 floor coverings – Environmental product declarations –
DIN EN 1307: 2014+A1:2016+A2:2018-05: Textile Product category rules
floor coverings - Classification
ISO 10874
EN 13501-1 DIN EN ISO 10874: 2012+A1:2021-04: Resilient,
DIN EN 13501-1:2019-05: Fire classification of textile and laminate floor coverings - Classification
construction products and building elements - Part 1:
Classification using data from reaction to fire tests ISO 14025
DIN EN /ISO 14025:2011-10/, Environmental labels
EN 14041 and declarations — Type III environmental
DIN EN 14041: 2018-05 and DIN EN 14041: 2008-05: declarations — Principles and procedures
Resilient, textile and laminate floor coverings -
Essential characteristics
ISO 14040
EN 15804 DIN EN ISO 14040:2006+A1:2020 Environmental
DIN EN 15804:2012+A2:2019 + AC:2021, management - Life cycle assessment - Principles and
Sustainability of construction works — Environmental framework
Product Declarations — Core rules for the product
category of construction products ISO 14044
DIN EN ISO 14044:2006+A1:2018+A2:2020
EN 16810 Environmental management - Life cycle assessment -
DIN EN 16810: 2017-08: Resilient, textile and laminate Requirements and guidelines
7 Environmental Product Declaration Interface – Tufted tiles, 75% rec. PA 6.6 with a maximum total pile weight of 1000
g/m2 , CQuest Bio Sone+ backing
ISO 15686 GaBi database
ISO 15686: Buildings and constructed assets - GaBi Software-System and Database for Life Cycle
Service life planning Engineering, version 10.5 Sphera, Leinfelden-
ISO 15686-1: 2011-05: Part 1: General principles and Echterdingen, database version 2022-1
framework
ISO 15686-2: 2012-05: Part 2: Service life prediction PCR Part A
procedures Product Category Rules for Building-Related Products
ISO 15686-7: 2017-04: Part 7: Performance and Services Part A: Calculation Rules for the Life
evaluation for feedback of service life data Cycle Assessment and Requirements on the Project
from practice Report according to EN 15804+A2:2019, V1.2, Berlin:
ISO 15686-8: 2008-06: Part 8: Reference service life Institut Bauen und Umwelt e.V. (IBU), November 2021
and service-life estimation
PCR Part B
Regulation (EU) No. 305/2011 Product Category Rules for Building-Related Products
Regulation No. 305/2011 Construction Products and Services
Regulation (CPR) of the European Council and of the Part B: Requirements on the EPD for floor coverings,
European Parliament, April 2011 V1.2, Berlin: Institut Bauen und Umwelt e.V. (IBU),
February 2018
General Instructions for the IBU-EPD Program
General Instructions for the EPD-Program of the PRODIS
Institut Bauen und Umwelt e.V., The Preparation of Product Information System (PRODIS) of the
Environmental Product Declarations - EPDs, version European Carpet Industry, Gemeinschaft
2.0, Institut Bauen und Umwelt e.V., Berlin, January umweltfreundlicher Teppichboden e.V (GUT) and
2021, www.ibu-epd.de European Carpet and Rug Association
(ECRA), http://www.pro-dis.info
BNB, Nutzungsdauer von Bauteilen
Bewertungssystem Nachhaltiges Bauen (BNB), REACH
Nutzungsdauer von Bauteilen, Bundesministerium des Regulation (EC) No 1907/2006 of the European
Inneren, für Bau und Heimat, 24.02.2017 Parliament and of the Council of 18 December 2006
concerning the Registration, Evaluation, Authorisation
ECHA candidate list and Restriction of Chemicals (REACH), June 2017,
Candidate List of substances of very high concern last update: 08.07.2021
(SVHCs) for authorisation, 08.07.2021, European
Chemicals Agency (ECHA), Helsinki, Finland VDZ e.V.
Association of German Cement Works, Ed. Environ-
mental Data of the German Cement Industry 2020
ecoinvent
ecoinvent, Zurich, Switzerland, database version 3.7,
published September 2020
8 Environmental Product Declaration Interface – Tufted tiles, 75% rec. PA 6.6 with a maximum total pile weight of 1000
g/m2 , CQuest Bio Sone+ backing
Publisher
Institut Bauen und Umwelt e.V. Tel +49 (0)30 3087748- 0
Hegelplatz 1 Fax +49 (0)30 3087748- 29
10117 Berlin Mail info@ibu-epd.com
Germany Web www.ibu-epd.com
Programme holder
Institut Bauen und Umwelt e.V. Tel +49 (0)30 - 3087748- 0
Hegelplatz 1 Fax +49 (0)30 – 3087748 - 29
10117 Berlin Mail info@ibu-epd.com
Germany Web www.ibu-epd.com
Author of the Life Cycle
Assessment Tel +49 (0)241 96843 410
Gemeinschaft umweltfreundlicher Fax +49 (0)241 96843 400
Teppichboden (GUT) e.V. Mail mail@gut-ev.de
Schönebergstraße 2 Web www.gut-ev.org
52068 Aachen
Germany
Owner of the Declaration
Interface Europe Manufacturing Tel +31 33 277 55 55
BV Fax +31 33 277 55 54
Industrielaan 15 Mail receptie@interface.com
3925ZG Scherpenzeel Web www.interface.com
Netherlands
