ENVIRONMENTAL PRODUCT DECLARATION
as per ISO 14025 and EN 15804+A2
Owner of the Declaration DORMA Hüppe Raumtrennsysteme GmbH
Publisher Institut Bauen und Umwelt e.V. (IBU)
Programme holder Institut Bauen und Umwelt e.V. (IBU)
Declaration number EPD-DHR-20240217-IBA1-EN
Issue date 03.07.2024
Valid to 02.07.2029
VARIFLEX 88/100 Movable Wall System
DORMA Hüppe
www.ibu-epd.com | https://epd-online.com
General Information
DORMA Hüppe VARIFLEX 88/100 Movable Wall System
Programme holder Owner of the declaration
IBU – Institut Bauen und Umwelt e.V. DORMA Hüppe Raumtrennsysteme GmbH
Hegelplatz 1 Industriestraße 5
10117 Berlin 26655 Westerstede/ Ocholt
Germany Germany
Declaration number Declared product / declared unit
EPD­DHR­20240217­IBA1­EN 1 m2 of the product: VARIFLEX 100 consisting of the following items:
• Wall element
• Particle board with finish
• Product packaging
This declaration is based on the product category rules: Scope:
Room partition systems, 01.08.2021 This Environmental Product Declaration refers to a specific movable wall
(PCR checked and approved by the SVR) system manufactured by DORMA Hüppe. The production site is located in
Westerstede/Ocholt (Germany).
Issue date Green electricity with Guarantee of Origin (GoO) is being used at this
production site.
03.07.2024
The data represents the year 2023.
Valid to
The owner of the declaration shall be liable for the underlying information
02.07.2029 and evidence; the IBU shall not be liable with respect to manufacturer
information, life cycle assessment data and evidences.
The EPD was created according to the specifications of EN 15804+A2. In
the following, the standard will be simplified as EN 15804.
Verification
The standard EN 15804 serves as the core PCR
Independent verification of the declaration and data according to ISO
14025:2011
internally X externally
Dipl.­Ing. Hans Peters
(Chairman of Institut Bauen und Umwelt e.V.)
Florian Pronold Matthias Klingler,
(Managing Director Institut Bauen und Umwelt e.V.) (Independent verifier)
1 Environmental Product Declaration ­ DORMA Hüppe ­ VARIFLEX 88/100 Movable Wall System
Product
Name Value Unit
Product description/Product definition
Sound reduction index to ISO 10140 39­59 dB
The VARIFLEX 88/100 room partition system is a horizontally
Heat transition coefficient to ISO 6946 0.4 ­ 0.59 W/(m²K)
movable sound insulated partition wall system made of steel
and aluminum, comprising individual elements which can be Load from wall weight 0.36­ 0.59 kN/m²
moved independently. A wide variety of design options is Performance data of the product with respect to its
possible. The cover panels are acoustically self­supporting. An characteristics in accordance with the relevant technical
element height of up to 14.5 meters can be realized. provision which can be applied are mentioned above.
For the Variflex 88/100 the standards which can be applied are
the following:
Base materials/Ancillary materials
• DIN 18032-3 The major material composition including the packaging of the
• EN 16516 product (m2) is listed below:
• ISO 6946 Name Value Unit
• ISO 9001 Particle board 50 %
• ISO 10140
Bitumen foil 21 %
• ISO 14001
Steel 17 %
• ISO 22196
• 2001/118/EC Aluminum 5 %
• AgBB 2021 Glass wool 2 %
• WECOBIS 2012 Plastics 3 %
Cast zinc 1 %
The CE­marking takes into account the proof of conformity with
Paper 1 %
the respective harmonized standards based on the legal
provisions above. The Variflex 88/100 Movable Wall Systems include partial
articles which contain substances listed in the Candidate List of
REACH Regulation 1907/2006/EC (date: 23.01.2024)
Application exceeding 0.1 percentage by mass: no
Areas of application include:
• Offices The Candidate List can be found on the ECHA website
• Hotels address: https:echa.europa.eu/de/home.
• Conference centers
• Trade fairs
• Schools
Reference service life
• Religious institutions
The reference service life of the VARIFLEX 88/100 is about 25
• Ateliers
years, depending on the application and frequency of use
Technical Data (approx. 50 closing cycles per year). For repairs and renewals,
The VARIFLEX 88/100 has following technical properties: suitable spare parts are available.
LCA: Calculation rules
transport to the manufacturer, — A3, manufacturing and
Declared Unit assembly including provision of all materials, products and
The declared unit is 1 m2 of the product: VARIFLEX 88/100 energy (green electricity with Guarantee of Origin (GoO)), as
including packaging. well as waste processing up to the end­of­waste state.
Name Value Unit
Declared unit 1 m2 Construction stage - Modules A4-A5
The construction process stage includes: — A4, transport to the
Grammage 48.27 kg/m2
building site; — A5, installation into the building; including
Layer thickness 0.1 m provision of all materials, products and energy, as well as waste
Mass of declared Product 48,27 kg/m² processing up to the end­of­waste state or disposal of final
residues during the construction process stage.
Other declared units are allowed if the conversion is shown
transparently.
End-of-life stage– Modules C1-C4 and D
The end­of­life stage includes: — C1, de­construction,
System boundary demolition: — C2, transport to waste processing; — C3, waste
processing for reuse, recovery and/or recycling; — C4,
The type of EPD is: cradle to gate with options, modules C1–
disposal; including provision and all transport, provision of all
C4, and module D (A1–A3 + C + D and additional modules: A4
materials, products and related energy and water use. Module
+ A5)
D (Benefits and loads beyond the system boundary) includes:
— D, recycling potentials, expressed as net impacts and
Production - Module A1-A3
benefits.
The product stage includes: — A1, raw material extraction,
processing and mechanical treatments, processing of
secondary material input (e.g. recycling processes), — A2,
2 Environmental Product Declaration ­ DORMA Hüppe ­ VARIFLEX 88/100 Movable Wall System
Geographic Representativeness Comparability
Land or region, in which the declared product system is Basically, a comparison or an evaluation of EPD data is only
manufactured, used or handled at the end of the product´s possible if all the data sets to be compared were created
lifespan: Global according to EN 15804 and the building context, respectively
the product­specific characteristics of performance, are taken
into account. Background database: GaBi, SP40.
LCA: Scenarios and additional technical information
Reference service life
Characteristic product properties of biogenic carbon
Name Value Unit
Name ValueUnit
Life Span according to the manufacturer 25 a
kg
Biogenic carbon content in product 12.2
C
End of life (C1-C4)
Biogenic carbon content in accompanying kg
12.2 C1: The product dismantling from the building is done manually
packaging C
without environmental burden.
C2: Transport to waste management is 50 km.
Note: 1 kg of biogenic carbon is equivalent to 44/12 kg of CO2 Name Value Unit
Transport to the building site (A4) Collected separately waste type waste type 48.27 kg
Name Value Unit Recycling 8.97 kg
Litres of fuel 0.00276 l/100km Energy recovery 31.5 kg
Transport distance 100 km Landfilling 1.55 kg
Capacity utilization (including empty runs) 55 % The product is disassembled in a recycling process. Material
The product is transported via truck. The product is produced recycling is then assumed for metals. The plastic components
project specific in the DORMA Hüppe factory in and wood are assumed to be incinerated with energy recovery.
Westerstede/Ocholt in Germany. The main distribution regions Glass wool is sent to landfill. Region for the End of Life is:
are Germany, Austria, UK, France and Switzerland. In order to Global.
allow scaling to a specific point of installation 100 km are
declared. Reuse, recovery and/or recycling potentials (D), relevant
scenario information
Installation into the building (A5) Name Value Unit
Name Value Unit Recycling 100 %
Waste packaging (paper and plastic) 33,7 Kg The collection rate is 100%.
3 Environmental Product Declaration ­ DORMA Hüppe ­ VARIFLEX 88/100 Movable Wall System
LCA: Results
DESCRIPTION OF THE SYSTEM BOUNDARY (X = INCLUDED IN LCA; MND = MODULE OR INDICATOR NOT DECLARED; MNR
= MODULE NOT RELEVANT)
Benefits and
Construction loads beyond
Product stage Use stage End of life stage
process stage the system
boundaries
la ire ta m w a Ry lp p u s tro p s n a rT g n iru tc a fu n a M e h t m o rf tro p s n a rTe tis e h t o t e ta g y lb m e s s A e s U e c n a n e tn ia M ria p e R tn e m e c a lp e R tn e m h s ib ru fe R y g re n e la n o ita re p Oe s u re ta w la n o ita re p Oe s u n o itc u rts n o c ­e Dn o itilo m e d tro p s n a rT g n is s e c o rp e ts a W la s o p s iD ­e s u e R­y re v o c e R­g n ilc y c e Rla itn e to p
A1 A2 A3 A4 A5 B1 B2 B3 B4 B5 B6 B7 C1 C2 C3 C4 D
X X X X X MND MND MNR MNR MNR MND MND X X X X X
RESULTS OF THE LCA - ENVIRONMENTAL IMPACT according to EN 15804+A2: 1 m2 Variflex 88/100 Movable Wall System
Parameter Unit A1-A3 A4 A5 C1 C2 C3 C4 D
GWP­total kg CO 2 eq 2.5E+01 7.17E­01 5.82E+01 0 2.11E­01 7.75E+01 2.37E­02 ­7.92E+01
GWP­fossil kg CO 2 eq 1.06E+02 6.85E­01 1.31E+01 0 2.02E­01 3.16E+01 2.35E­02 ­7.9E+01
GWP­biogenic kg CO 2 eq ­8.12E+01 3.17E­02 4.51E+01 0 9.33E­03 4.59E+01 8.03E­05 ­2.01E­01
GWP­luluc kg CO 2 eq 1.19E­01 1.63E­05 1.3E­03 0 4.8E­06 2.19E­03 6.77E­05 ­4.72E­02
ODP kg CFC11 eq 6.43E­10 7.23E­17 1.31E­14 0 2.13E­17 2.12E­14 8.72E­17 ­7.11E­11
AP mol H+ eq 4.97E­01 6.86E­04 1.07E­02 0 2.02E­04 1.22E­02 1.69E­04 ­1.91E­01
EP­freshwater kg P eq 4.43E­04 1.47E­07 2.22E­06 0 4.32E­08 3.33E­06 4.04E­08 ­1.22E­04
EP­marine kg N eq 9.17E­02 2.18E­04 3.05E­03 0 6.43E­05 3.41E­03 4.34E­05 ­3.47E­02
EP­terrestrial mol N eq 1.07E+00 2.43E­03 4.53E­02 0 7.14E­04 5.65E­02 4.77E­04 ­3.72E­01
kg NMVOC
POCP 2.75E­01 6.17E­04 8.32E­03 0 1.82E­04 9.33E­03 1.31E­04 ­1.11E­01
eq
ADPE kg Sb eq 2.12E­02 2.06E­08 1.94E­07 0 6.05E­09 3.04E­07 2.11E­09 ­7.82E­03
ADPF MJ 2.07E+03 9.72E+00 1.77E+01 0 2.86E+00 2.43E+01 3.08E­01 ­1.24E+03
m3 world eq
WDP 1.12E+02 1.34E­03 6.4E+00 0 3.95E­04 7.96E+00 2.46E­03 ­9.26E+00
deprived
GWP = Global warming potential; ODP = Depletion potential of the stratospheric ozone layer; AP = Acidification potential of land and water; EP =
Eutrophication potential; POCP = Formation potential of tropospheric ozone photochemical oxidants; ADPE = Abiotic depletion potential for non­fossil
resources; ADPF = Abiotic depletion potential for fossil resources; WDP = Water (user) deprivation potential)
RESULTS OF THE LCA - INDICATORS TO DESCRIBE RESOURCE USE according to EN 15804+A2: 1 m2 Variflex 88/100
Movable Wall System
Parameter Unit A1-A3 A4 A5 C1 C2 C3 C4 D
PERE MJ 8.17E+02 3.06E­02 3.75E+02 0 9.02E­03 4.65E+02 4.04E­02 ­2.93E+02
PERM MJ 8.3E+02 0 ­3.71E+02 0 0 ­4.59E+02 0 0
PERT MJ 1.65E+03 3.06E­02 3.72E+00 0 9.02E­03 5.58E+00 4.04E­02 ­2.93E+02
PENRE MJ 1.84E+03 9.73E+00 2.24E+02 0 2.86E+00 5E+01 3.09E­01 ­1.24E+03
PENRM MJ 2.32E+02 0 ­2.06E+02 0 0 ­2.57E+01 0 0
PENRT MJ 2.07E+03 9.73E+00 1.77E+01 0 2.86E+00 2.43E+01 3.09E­01 ­1.24E+03
SM kg 1.93E+00 0 0 0 0 0 0 0
RSF MJ 0 0 0 0 0 0 0 0
NRSF MJ 0 0 0 0 0 0 0 0
FW m3 2.87E+00 5.5E­05 1.51E­01 0 1.62E­05 1.88E­01 7.78E­05 ­4.39E­01
PERE = Use of renewable primary energy excluding renewable primary energy resources used as raw materials; PERM = Use of renewable primary
energy resources used as raw materials; PERT = Total use of renewable primary energy resources; PENRE = Use of non­renewable primary energy
excluding non­renewable primary energy resources used as raw materials; PENRM = Use of non­renewable primary energy resources used as raw
materials; PENRT = Total use of non­renewable primary energy resources; SM = Use of secondary material; RSF = Use of renewable secondary fuels;
NRSF = Use of non­renewable secondary fuels; FW = Use of net fresh water
RESULTS OF THE LCA – WASTE CATEGORIES AND OUTPUT FLOWS according to EN 15804+A2:
1 m2 Variflex 88/100 Movable Wall System
Parameter Unit A1-A3 A4 A5 C1 C2 C3 C4 D
HWD kg 7.14E­06 9.43E­10 3.67E­08 0 2.78E­10 6.15E­08 4.7E­09 ­7.98E­06
NHWD kg 7.55E+00 9.94E­04 2.25E+00 0 2.93E­04 3.54E+00 1.55E+00 ­2.09E+00
RWD kg 6.82E­02 1.04E­05 8.75E­04 0 3.07E­06 1.1E­03 3.51E­06 ­8.93E­02
CRU kg 0 0 0 0 0 0 0 0
MFR kg 0 0 0 0 0 8.97E+00 0 0
MER kg 0 0 0 0 0 0 0 0
EEE MJ 0 0 8.74E+01 0 0 1.24E+02 0 0
EET MJ 0 0 1.69E+02 0 0 2.52E+02 0 0
4 Environmental Product Declaration ­ DORMA Hüppe ­ VARIFLEX 88/100 Movable Wall System
HWD = Hazardous waste disposed; NHWD = Non­hazardous waste disposed; RWD = Radioactive waste disposed; CRU = Components for re­use;
MFR = Materials for recycling; MER = Materials for energy recovery; EEE = Exported electrical energy; EET = Exported thermal energy
RESULTS OF THE LCA – additional impact categories according to EN 15804+A2-optional:
1 m2 Variflex 88/100 Movable Wall System
Parameter Unit A1-A3 A4 A5 C1 C2 C3 C4 D
Disease
PM 8.91E­06 3.61E­09 8.29E­08 0 1.06E­09 1.04E­07 2.09E­09 ­2.25E­06
incidence
IR kBq U235 eq 8.18E+00 1.49E­03 1.23E­01 0 4.39E­04 1.38E­01 3.61E­04 ­1.45E+01
ETP­fw CTUe 1.41E+03 6.89E+00 7.83E+00 0 2.03E+00 9.73E+00 1.76E­01 ­3.34E+02
HTP­c CTUh 2.11E­07 1.3E­10 5.97E­10 0 3.81E­11 7.54E­10 2.61E­11 6.45E­08
HTP­nc CTUh 4.25E­06 5.54E­09 4.34E­08 0 1.63E­09 5.72E­08 2.88E­09 8.3E­06
SQP SQP 7.51E+03 2.5E­02 5.01E+00 0 7.35E­03 7.07E+00 6.43E­02 ­1.48E+02
PM = Potential incidence of disease due to PM emissions; IR = Potential Human exposure efficiency relative to U235; ETP­fw = Potential comparative
Toxic Unit for ecosystems; HTP­c = Potential comparative Toxic Unit for humans (cancerogenic); HTP­nc = Potential comparative Toxic Unit for humans
(not cancerogenic); SQP = Potential soil quality index
Disclaimer 1 – for the indicator “Potential Human exposure efficiency relative to U235”. This impact category deals mainly with the
eventual impact of low­dose ionizing radiation on human health of the nuclear fuel cycle. It does not consider effects due to possible
nuclear accidents, occupational exposure or radioactive waste disposal in underground facilities. Potential ionizing radiation from the
soil, radon and from some construction materials is also not measured by this indicator.
Disclaimer 2 – for the indicators “abiotic depletion potential for non­fossil resources”, “abiotic depletion potential for fossil resources”,
“water (user) deprivation potential, deprivation­weighted water consumption”, “potential comparative toxic unit for ecosystems”,
“potential comparative toxic unit for humans – cancerogenic”, “Potential comparative toxic unit for humans ­ not cancerogenic”,
“potential soil quality index”. The results of this environmental impact indicator shall be used with care as the uncertainties on these
results are high as there is limited experience with the indicator.
This EPD was created using a software tool.
References
EN 15804 airborne sound insulation
EN 15804+A2:2019+AC:2021, Sustainability of construction
works — Environmental Product Declarations — Core rules for ISO 14001
the product category of construction products ISO 14001:2015 Environmental Management System
ECHA ISO 22196
European Chemical Agency ISO 22196:2011­08 Measurement of antibacterial activity on
plastic and other non­porous surfaces
ISO 14025
ISO 14025:201110, Environmental labels and declarations — 2001/118/EC
Type III environmental declarations — Principles and European Waste Catalogue (EWC) – Commission decision of
procedures 16 January 2001 amending Decision 2000/532/EC as regards
the list of wastes
REACH
Regulation (EC) No 1907/2006 of the European Parliament and AgBB 2021
of the Council on the Registration, Evaluation, Authorization AgBB 2021 Health­related Evaluation of Volatile Organic
and Restriction of Chemicals (REACH) Compounds (VVOC, VOC and SVOC) from Building Products
Further References WECOBIS 2012
WECOBIS 2012 Ecological building material information
DIN 18032 system, German Ministry of Transport, Building and Urban
DIN 18032­3:1997­04, Testing of safety against ball throwing Affairs
EN 16516 IBU 2021
EN 16516 ­ 2020­10 Construction products: Testing and General Instructions for the EPD programme of Institut Bauen
evaluation of the release of dangerous substances ­ und Umwelt e.V. Version 2.0, Berlin: Institut Bauen und Umwelt
Determination of emissions into indoor air e.V., 2021. www.ibu­epd.com
ISO 6946 GaBi
ISO 6946:2008­04, Thermal resistance and thermal Sphera Solutions GmbH
transmittance ­ Calculation method Gabi Software System and Database for Life Cycle Engineering
19922020
ISO 9001 Version 10.0.0.71
ISO 9001:2015­11, Quality management systems ­ University of Stuttgart
Requirements Leinfelden­Echterdingen
ISO 10140 GaBi ts documentation
ISO 10140­2:2010­12, Acoustics ­ Laboratory measurement of GaBi life cycle inventory data
sound insulation of building elements ­ Part 2: Measurement of documentation
5 Environmental Product Declaration ­ DORMA Hüppe ­ VARIFLEX 88/100 Movable Wall System
(https://www.gabisoftware.com/support/gabi/gabidatabase­ according to EN 15804+A2:2019, Version 1.0, 2020, Institut
2020­lci documentation/) Bauen und Umwelt e.V., www.ibu­epd.com
dormakaba LCA-tool PCR Part B
LCA tool, Tool No.: IBU­­DOR­­202106­­LT1­­EN, developed by PCR – Part B: Requirements on the EPD for Room partition
SpheraSolutions GmbH systems, version 08/2021, Institut Bauen und Umwelt e.V.,
www.ibu­epd.com
PCR Part APCR – Part A: Calculation Rules for the Life Cycle
Assessment and Requirements on the Project Re­port
6 Environmental Product Declaration ­ DORMA Hüppe ­ VARIFLEX 88/100 Movable Wall System
Publisher
Institut Bauen und Umwelt e.V. +49 (0)30 3087748­ 0
Hegelplatz 1 info@ibu­epd.com
10117 Berlin www.ibu­epd.com
Germany
Programme holder
Institut Bauen und Umwelt e.V. +49 (0)30 3087748­ 0
Hegelplatz 1 info@ibu­epd.com
10117 Berlin www.ibu­epd.com
Germany
Author of the Life Cycle Assessment
dormakaba International Holding GmbH +49 2333 793­0
DORMA Platz 1 info.de@dormakaba.com
58256 Ennepetal www.dormakaba.com
Germany
Owner of the Declaration
DORMA Hüppe Raumtrennsysteme GmbH +49 4409 6660
Industriestraße 5 info­hueppe@dormakaba.com
26655 Westerstede/ Ocholt www.dorma­hueppe.com
Germany
7 Environmental Product Declaration ­ DORMA Hüppe ­ VARIFLEX 88/100 Movable Wall System
