ENVIRONMENTAL PRODUCT DECLARATION
as per ISO 14025 and EN 15804+A2
Owner of the Declaration Moland Group A/S
Publisher Institut Bauen und Umwelt e.V. (IBU)
Programme holder Institut Bauen und Umwelt e.V. (IBU)
Declaration number EPD-MOL-20230148-IBA1-EN
Issue date 29.08.2023
Valid to 28.08.2028
Moland Super Eg
Moland Group A/S
www.ibu-epd.com | https://epd-online.com
1. General Information
Moland Group A/S Moland Super Eg
Programme holder Owner of the declaration
IBU – Institut Bauen und Umwelt e.V. Moland Group A/S
Hegelplatz 1 Strandvejen 16
10117 Berlin 7800 Skive
Germany Denmark
Declaration number Declared product / declared unit
EPD-MOL-20230148-IBA1-EN 1 m² of veneered, wood flooring with HDF carrier (10 mm)
This declaration is based on the product category rules: Scope:
Solid wood products, 01.08.2021 This Environmental Product Declaration covers an average square meter
(PCR checked and approved by the SVR) of pre-lacquered, veneered, wood flooring with HDF carrier (10 mm),
produced by Moland Group A/S in Denmark.
The owner of the declaration shall be liable for the underlying information
Issue date and evidence; the IBU shall not be liable with respect to manufacturer
information, life cycle assessment data and evidences.
29.08.2023
The EPD was created according to the specifications of EN 15804+A2. In
the following, the standard will be simplified as EN 15804.
Valid to
28.08.2028 Verification
The standard EN 15804 serves as the core PCR
Independent verification of the declaration and data according to ISO
14025:2011
internally X externally
Dipl.-Ing. Hans Peters
(Chairman of Institut Bauen und Umwelt e.V.)
Florian Pronold Dr. Matthew Fishwick,
(Managing Director Institut Bauen und Umwelt e.V.) (Independent verifier)
1 Environmental Product Declaration - Moland Group A/S - Moland Super Eg
2. Product
Name Value Unit
2.1 Product description/Product definition
Moisture content acc. to EN 322 5-9 %
Moland Super Eg is a multi-layered parquet, consisting of a
Mean density 850 kg/m³
wood wear layer, pressed onto high-density fibreboard (HDF)
with a wooden backing. Moland Super Eg floors are finished Thickness 10 mm
with a top layer of authentic wood species, sourced from Length 593 - 2050 mm
responsible forestry. The thickness of the veneer top layer is Width 121 - 233 mm
0.6 mm in order to make the most of the material.
Reaction to fire EN 13501-1 Cfl-s1 Class
Formaldehyde emission EN 717-1 E1 Class
The thin veneer layer of 0.6 mm is pressed on the HDF board
according to the DSI (Double-Sided Impregnation) system. Content PCP EN 14342 < 5 ppm
During this process, the adhesive is pressed into and absorbed Slip resistance CEN/TS 15676 ≥ 45 USRV
by the wood. Thermal conductivity EN 12667 0.14 W/mK
Installation method floating -
The surface finish, consisting of eight robust layers of specially
developed lacquers protects the floor from wear and tear as Performance data of the product in accordance with the
well as scratches. The wood absorbs the varnish which fuses declaration of performance with respect to its essential
with the adhesive. This results in a high-strength and scratch- characteristics according to EN 14342:2013, Wood flooring and
resistant floor and a moist and dirt-resistant surface. parquet - Characteristics, evaluation of conformity and marking.
Verification and assessment of constancy of performance are
The combination of the thin top layer, the high-densitiy carried out according to system 3.
fibreboard and the wooden backing ensures impact resistance
2.4 Delivery status
and dimensional stability. Moland Super Eg floors are equipped
All products are delivered in packaging units. The following
with a click system for easy installation.
information is specified on the box:
For the placing on the market of the product in the European • Finish
Union/European Free Trade Association (EU/EFTA) (with the • Wood type
exception of Switzerland) Regulation (EU) No. 305/2011 (CPR) • Box quantity [m²]
applies. The product needs a declaration of performance taking • Dimensions [mm]
into consideration EN 14342:2013 Wood flooring and parquet - • Number of parquet planks [pcs]
Characteristics, evaluation of conformity and marking as well as
the CE-marking. Further specification is according to EN Dimensions of the declared products as delivered are within
14354:2017, the European standard for wood veneer floor following ranges:
coverings, as referenced by EN 14342:2013. For the
• Length: 593 - 2050 mm
application and use., the respective national provisions apply.
• Width: 121 - 233 mm
• Thickness: 10 mm
2.2 Application
• Box quantity: 0.79 -2.39 m²
Moland Super Eg flooring is covered by harmonised standards,
EN 14342:2013 and EN 14354:2017. It's intended as floor 2.5 Base materials/Ancillary materials
covering for internal use in dry conditions. The provided click
The average composition of the finished products is calculated
system is only suitable for floating installations. Flooring without
per product group. The components of Moland Super Eg are
an integrated cork layer should be installed on a suitable
given below in kg/m² flooring.
underlay. Moland Super Eg flooring can be installed for both
private and commercial use. The installation must be carried • Lacquer < 1.5 %
out in accordance with the installation instructions, the rules of • Veneer (top layer & backing) 9 %
the trade and the state of the art. • Adhesive (UF-glue) < 1 %
• High-density fibreboard 89 %
2.3 Technical Data
Technical specifications in accordance with the information in This product/article/at least one partial article contains
the declaration of performance with respect to its essential substances listed in the candidate list (17.01.2023) exceeding
characteristics following EN 14342:2013, Wood flooring and 0.1 percentage by mass: No
parquet - Characteristics, evaluation of conformity and marking.
This product/article/at least one partial article contains other
Constructional data
carcinogenic, mutagenic, reprotoxic (CMR) substances in
categories 1A or 1B which are not on the candidate list,
exceeding 0.1 percentage by mass: No
Biocide products were added to this construction product or it
has been treated with biocide products (this then concerns a
treated product as defined by the (EU) Ordinance on Biocide
Products No. 528/2012): No
2.6 Manufacture
Moland Group A/S produces Moland Super Eg flooring at its
production site in Denmark. The production process mainly
involves assembly of the above, purchased components (HDF,
veneer, adhesive, lacquer). Prior to the assembly process, an
2 Environmental Product Declaration - Moland Group A/S - Moland Super Eg
extended part of the production is dedicated to the sorting,
preparing and jointing of the veneer. The health and safety manager keeps track of safe use
guidelines and provides appropriate personal protection
Veneer is produced by slicing a log into thin layers. This equipment when needed. Since air extraction systems filter
process makes optimal use of the logs because, in contrast ambient air in production, personal protection equipment mainly
with solid wood, there is no sawing loss. The purchased involves:
bundles of veneer are sorted and evaluated on various aspects:
• Protective clothing
• Wood species • Safety shoes
• Slicing technique • Hearing protection
• Dimensions • Gloves
• Quality All employees are provided with the above mentioned, suitable
After the assignment of a certain quality level, the bundles are protection measures.
cut in length and width. By using advanced technology, the
sliced wood can be joined into veneer sheets, which are again A committee for prevention and protection at work is in place.
graded, based on their quality. Training for personnel is carried out at regular intervals,
including: at the start of employment, annual recap or when
The next step in the production process is pressing. Adhesive is deemed necessary.
applied to both sides of the HDF carrier, which is subsequently All of this is captured in safety procedures, prevention and
placed onto the wooden backing. The wooden wear layer is protection reports and put into practice by means of e.g. fire
placed on top. By placing this combination of materials in the exercises, first aid training organized by the HR- and HSE-
press at a predefined time, temperature and pressure level, the manager.
adhesive is pressed into and absorbed by the wood. After
pressing, the veneered board is trimmed to the desired Chemical residues are sorted and collected separately. These
dimensions and subjected to quality control. containers are picked up by our waste processor and
processed according to applicable disposal regulations.
Finishing of the wooden wear layer is done by applying eight
layers of specially developed lacquers. Prior to this process, the Environmental protection measures:
wooden wear layer is sanded and optionally brushed. The eight Moland Group A/S is Program for the Enforcement of Forest
layers of lacquer are cured by means of UV light. This Certification (PEFC) certified. This organisation is committed to
extremely strong and matt lacquer is nearly invisible. The responsible forest management and includes social aspects in
quality of the finishing process is extensively inspected. their policy. Wood or wood-based materials are responsibly
sourced with one of the above-mentioned certifications.
After approval of the finishing quality, the lacquered veneered Internal wood waste is incinerated with energy recovery which
boards are divided into parquet planks. Dimensions of the is re-used in the manufacturing process. Air extraction systems
planks depend on the collection. Each plank is provided with a filter ambient air in production. A committee for prevention and
click system, which is carefully milled to the sides. protection at work is in place.
The wooden flooring is packed in cardboard boxes and 2.8 Product processing/Installation
wrapped with plastic foil. Before starting the installation, it is essential to read the
installation instructions carefully. Moland Super Eg flooring is
At the end of the manufacturing process, a full quality intended for floating installation and can easily be installed, with
inspection check is performed and documented according to its click tongue-and-groove system. Following installation tools
the internal Factory Production Control (FPC) system. are recommended:
• Installation kit
• Pencil
• Meter
• Hammer
• Handsaw
• Cutter
Besides the above-mentioned installation tools, Moland Super
Eg flooring can be processed with all tools, suitable for solid
wood. These tools must be operated in accordance with the
manufacturer's operating instructions. Make sure that the
necessary safety precautions and protection measures (e.g.
hearing protection, respiratory mask, protective gloves, safety
glasses...) are applied. Provide adequate ventilation if the
processing operations generate wood dust.
2.7 Environment and health during manufacturing Dispose of the product and packaging in accordance with
Health protection measures applicable, local, or national disposal regulations.
Applicable legislation is strictly and fully applied. Working
2.9 Packaging
conditions comply with all requirements and in particular, with
regard to health and safety. Moland Super Eg flooring is packed in a cardboard box and
wrapped with PE-foil in order to protect the product during
Possible hazards, related to chemicals used in production, are transport and storage.
covered by a yearly due diligence exercise where material Packaging material must be collected separately and disposed
safety data sheets are collected and conformity with the of in accordance with applicable legislation.
REACH-regulation (incl. SVHC's) is evaluated.
3 Environmental Product Declaration - Moland Group A/S - Moland Super Eg
2.10 Condition of use 2.13 Extraordinary effects
Before installation, Moland Super Eg flooring should be stored Fire
in a dry and protected room with an air humidity of 40 – 60 % Moland Super Eg, wood veneered floor covering, with surface
and a temperature between 16-21°C. Wood has, as a coating and with or without cork bottom layer is classified as
hygroscopic material, the ability to absorb and release moisture Cfl-s1. Test conditions: in accordance with EN 13501-1:2019 .
from the surrounding environment. Changes in moisture Installation method: loose-laid on end-use substrates of wood
content can result in dimensional changes over time. This and of classes A1 and A2-s1,d0.
needs to be accommodated during installation by foreseeing
Fire protection
expansion gaps of 1 mm per running meter, as outlined in the
Name Value
installation instructions.
Building material class Cfl
2.11 Environment and health during use Smoke gas development s1
The use phase of Moland Super Eg flooring is not in the scope
of the Life Cycle Assessment (LCA) and resulting EPD.
Water
However, measurements of VOC emissions to indoor air are
Moland Super Eg flooring has a water-resistant surface but is
measured and available.
not able to withstand prolonged exposure to water. Besides
Moland Super Eg flooring complies with following regulations
damage to the product, no adverse consequences to the
and test protocols:
environment will occur.
• Indoor Air Comfort GOLD®
• CDPH Mechanical destruction
• M1 No negative impacts on the environment are identified when
Additional and more detailed information can be provided on mechanically destroying the product. Suitable personal
request. Moland Super Eg flooring does not imply any hazards protection equipment is recommended to prevent injury or
to water, air or soil when used as intended. health risks, caused by sharp edges, wood chips or wood dust.
2.12 Reference service life 2.14 Re-use phase
The service life in accordance with the Bundsinstitut fûr Stadt- Limited mechanical damage like scratches can be repaired
und Raumforschung (BBSR), table "Service lives of using the Repair Pens and Repair Wax. Colour and lacquer
components for life cycle assessment according to pens are available to repair the floor and to protect it from dirt
Bewertungssystem Nachhaltiges Bauen (BNB)", is and moisture.
• 40 years for wooden, multilayer parquet.
• 15 years for wood lacquers When your floor is severely damaged, the Bulldog allows you to
The service life is specified on an informative basis and is remove and replace the damaged plank(s). More information
based on the warranty period Moland Group A/S specifies for and instructions for use are available on www.moland.dk.
the products:
At end-of-life, the product can be incinerated with energy
recovery.
2.15 Disposal
Molan Super Eg flooring is classified as wood waste with EWC-
code 17 02 01, according to EUROSTAT Guidance.
The product must be disposed of in accordance with applicable,
The following information, related to maintenance and repair is
local or national disposal regulations.
informative, given that module B is not declared. The product
must be installed and maintained according to the installation 2.16 Further information
and maintenance instructions.
Additional information, contact details, installation and
Misuse or poor maintenance will adversely affect the service
maintenance instructions are available on www.moland.dk
life. This also applies for unusually low or high humidity,
excessive water use, dragging heavy furniture, etc.
3. LCA: Calculation rules
Name Value Unit
3.1 Declared Unit
Declared unit 1 m²
The declared unit is 1 m² of pre-lacquered, veneered wood
flooring with HDF carrier of 10 mm. The total inputs, outputs
Gross density 850 kg/m3
and produced m² for the period under consideration are taken Grammage 9.49 kg/m2
as a basis. Wood moisture at delivery 5 - 9 %
Layer thickness (Weighted averged thickness) 0.01 m
The products in this EPD represent an average in a product
group. The most important variable which leads to differences Moland Group A/S collected data for a full production year:
in the environmental profiles within the group is the amount of 2021. More specifically:
HDF in the product. For Moland Super Eg, the difference is • Raw material use and transport to the production
5.88 %. location
Declared unit • Relevant suppliers were contacted for primary data
• Energy use
• Emissions
• Production
4 Environmental Product Declaration - Moland Group A/S - Moland Super Eg
at industrial furnace >100 kW |Cut-off".
3.2 System boundary
This EPD is a cradle-to-gate with options (C1-C4, D) Since the LCA is based on production information from a full
production year it is expected that mass and energy balance is
Product stage A1-A3 (in) close (proximity) to complete as no materials or processes
Parquet consists of a high-density fibreboard to which a have been excluded. The cut-off criteria are well below 1 %.
wooden veneer layer is applied (glued) on both sides. All the
raw materials are supplied by truck. The application of veneer 3.5 Background data
onto the baseboard is called the pressing process. This For background processes, the ecoinvent database v3.6
pressing is achieved by means of pressure, temperature and (allocation cut-off) has been used.
time. The panels are then sawn, sanded and varnished. After
varnishing, the boards are divided in planks and are provided 3.6 Data quality
with a click system so that they can be clipped into one another. Data quality and validation of economic flows
Moland Group A/S collected data on the production of parquet
The heat used in the production process is obtained from the for a full production year, 2021. More
incineration of part of the wood production waste. specifically:
• Raw material use and transport to the production
The proportion of the electricity demand covered by green location
electricity in the total electricity demand is 100 %. • Primary data for important products were requested
from suppliers
Transport to construction (A4) • Energy use
This module is not in the scope of this EPD. • Emissions
• Production waste
Construction process (A5)
This module is not in the scope of this EPD. The provided data was checked for plausibility. The quality and
representativeness are considered high. The products in this
Use phase (B) EPD represent an average in a product group. The most
This module is not in the scope of this EPD. However, the important variable which leads to differences in the
emissions to indoor air will be mentioned informatively in this environmental profiles within the group is the amount of HDF in
EPD. these products. For Moland Super Eg, this difference is 5,88 %.
Demolition C1 For background processes, the ecoinvent database v3.6
Parquet can be removed from the building in a manual process. (allocation cut-off) has been used.
It is anticipated that the environmental impact of this process is
neglectable. Data quality and validation of environmental inventories
Since the LCA is based on production information from a full
Recovery D production year it is expected that mass and energy balance is
This module includes the benefit of the recovery of electricity close to complete. For the LCA calculations, the following
and heat that often occurs in waste incineration plants. For the methods have been used:
electrical and thermal efficiency of the waste-to-energy plant we
• SimaPro's LCA method: "EN 15804+A2" via
calculated with 18 % and 31 % respectively. For the heat of
bepalingsmethode 'set 1', 'set 2' & param (NMD 3.4)
combustion of parquet (wood) the lower heating value was
(see appendix C)
used: Wood: 13.99 MJ/kg.
SGS INSTRON has checked potential uncharacterised
3.3 Estimates and assumptions substances. This check is part of the validation of
Transport to waste treatment C2 environmental inventories.
After the parquet is removed from the application is transported
3.7 Period under review
to a waste treatment facility. In the waste treatment scenario in
The production data for this EPD is based on the production of
this LCA, a transport distance of 50 km is assumed.
a full production year (2021).
Waste processing C3
The waste treatment scenario in this study assumes that at the 3.8 Geographic Representativeness
waste treatment facility the parquet is chipped into wood chips.
Land or region, in which the declared product system is
Final waste treatment C4
manufactured, used or handled at the end of the product´s
The waste treatment scenario in this study assumes that that
lifespan: Denmark
the wood chips are used for incineration with energy recovery.
3.4 Cut-off criteria
3.9 Allocation
Emissions for the combustion of wood are not measured at the
The energy use for the production processes has been
plant and are therefore included via the ecoinvent used. There
allocated based on the area produced for each of the products.
is a process-specific emission to be expected from
The amount of production waste has been allocated based on
formaldehyde. The exact emission is not measured and
the mass of the products and the loss factor for each of the
therefore included based on the ecoinvent process "Glued
products.
laminated timber, for indoor use {RER}| production | Cut-off".
The emission included in the calculation is 0.0114 kg/m3 3.10 Comparability
product. The avoided production of electricity from primary Basically, a comparison or an evaluation of EPD data is only
sources is based on: "Electricity, high voltage {NL}|heat and possible if all the data sets to be compared were created
power co-generation, natural gas, combined cycle power plant, according to EN 15804 and the building context, respectively
400MWelectrical | Cut-off". The avoided production of heat from the product-specific characteristics of performance, are taken
primary sources is based on: "Heat, district or industrial, natural into account. For background processes, the ecoinvent
gas {Europe without Switzerland}| heat production, natural gas, database v3.6 (allocation cut-off) has been used.
5 Environmental Product Declaration - Moland Group A/S - Moland Super Eg
4. LCA: Scenarios and additional technical information
The service life is declared in accordance with the BBSR, table
Characteristic product properties of biogenic carbon "Service lives of components for life cycle assessment
The amount of biogenic C in the product has been calculated according to BNB".
using the amount of veneer, HDF and cork in the product,
Name Value Unit
multiplication by the wood and cardboard content and 0.5. The
Life span according to BBSR 15 years
latter is the amount of C in wood according to EN 16485:2014.
The wood content in HDF is 77 % according to the suppliers Life span according to the See section -
EPD: EPD-UNI-20150013-IBA1-EN. For veneer and cork, a manufacturer 2.12
moisture content of 6 % has been used.
End of life (C1-C4)
Note: 1 kg of biogenic carbon is equivalent to 44/12 kg of CO .
2
Information on describing the biogenic carbon content at Demolition C1
factory gate Parquet is typically removed from the building in a manual
Name ValueUnit process. It is anticipated that the environmental impact of this
kg process is neglectable.
Biogenic carbon content in product 3.67
C
Transport to waste treatment C2
Biogenic carbon content in accompanying kg
0.08 After the parquet is removed from the application it's
packaging C
transported to a waste treatment facility. In the waste treatment
scenario in this LCA a transport distance of 50 km is assumed
Use or application of the installed product (B1) see (ecoinvent: "Transport, freight, lorry, unspecified {GLO}| market
section 2.12 "Use" group for transport, freight, lorry, unspecified | Cut-off)".
This module is not in scope. However, the emissions to indoor
air are informatively mentioned in section 2.11. Waste processing (C3)
The waste treatment scenario in this study assumes that at the
The following information, related to maintenance and repair is waste treatment facility the parquet is chipped into wood chips.
informative, given that module B is not declared. The following ecoinvent process is used: "Wood chipping,
industrial residual wood, stationary electric chipper {GLO}|
Maintenance (B2) market for | Cut-off".
The specially developed Wood Floor Cleaner is recommended
to maintain the parquet. It removes dirt without harming the Final waste treatment (C4)
lacquer. Maintenance instructions are available on The waste treatment scenario in this study assumes that the
www.moland.dk wood chips are used for incineration with energy recovery. It is
assumed that the energy efficiency of energy recovery is 18 %
Repair (B3) electric and 31 % thermal. Since this efficiency is <60 %, the
Limited mechanical damage like scratches can be repaired incineration process is included in module C4.
using the Repair Pens and Repair Wax. Colour and lacquer
Name Value Unit
pens are available to repair the floor and protect it from dirt and
Collected separately waste type waste wood 9.49 kg
moisture.
Energy recovery 9.49 kg
Replacement (B4) / Refurbishment (B5)
When your floor is severely damaged, the Bulldog allows you to Reuse, recovery and/or recycling potentials (D), relevant
remove and replace the damaged plank(s). More information scenario information.
and instructions for use are available on www.moland.dk. The benefit of the recuperation of electricity and heat that often
Reference service life occurs in waste incineration plants was included in module D.
6 Environmental Product Declaration - Moland Group A/S - Moland Super Eg
5. LCA: Results
DESCRIPTION OF THE SYSTEM BOUNDARY (X = INCLUDED IN LCA; MND = MODULE OR INDICATOR NOT DECLARED; MNR
= MODULE NOT RELEVANT)
Benefits and
Construction loads beyond
Product stage Use stage End of life stage
process stage the system
boundaries
la ire ta m w a Ry lp p u s tro p s n a rT g n iru tc a fu n a M e h t m o rf tro p s n a rTe tis e h t o t e ta g y lb m e s s A e s U e c n a n e tn ia M ria p e R tn e m e c a lp e R tn e m h s ib ru fe R y g re n e la n o ita re p Oe s u re ta w la n o ita re p Oe s u n o itc u rts n o c -e Dn o itilo m e d tro p s n a rT g n is s e c o rp e ts a W la s o p s iD -e s u e R-y re v o c e R-g n ilc y c e Rla itn e to p
A1 A2 A3 A4 A5 B1 B2 B3 B4 B5 B6 B7 C1 C2 C3 C4 D
X X X MND MND MND MND MNR MNR MNR MND MND X X X X X
RESULTS OF THE LCA - ENVIRONMENTAL IMPACT according to EN 15804+A2: 1 m2 Veneered, wood flooring with HDF
carrier (10 mm) (10 mm)
Parameter Unit A1-A3 C1 C2 C3 C4 D
Global Warming Potential total (GWP-total) kg CO 2 eq -2.35E+00 0 1.32E-01 1.34E-01 1.7E+01 -6.35E-01
Global Warming Potential fossil fuels (GWP-fossil) kg CO 2 eq 1.43E+01 0 1.32E-01 1.33E-01 1.42E-01 -5.69E-01
Global Warming Potential biogenic (GWP-biogenic) kg CO 2 eq -1.68E+01 0 6.07E-05 1.04E-03 1.68E+01 -5.88E-02
Global Warming Potential luluc (GWP-luluc) kg CO 2 eq 1.9E-01 0 4.82E-05 2.39E-04 2.53E-05 -6.55E-03
Depletion potential of the stratospheric ozone layer (ODP) kg CFC11 eq 1.15E-06 0 2.9E-08 6.03E-09 1.14E-08 -1.67E-07
Acidification potential of land and water (AP) mol H+ eq 9.81E-02 0 7.63E-04 6.75E-04 1.6E-03 -1.85E-02
Eutrophication potential aquatic freshwater (EP-freshwater) kg P eq 1.9E-03 0 1.33E-06 8.1E-06 1.85E-06 -5.84E-05
Eutrophication potential aquatic marine (EP-marine) kg N eq 1.86E-02 0 2.69E-04 1.12E-04 7.54E-04 -5.42E-03
Eutrophication potential terrestrial (EP-terrestrial) mol N eq 2.1E-01 0 2.96E-03 1.28E-03 8.03E-03 -8.92E-02
Formation potential of tropospheric ozone photochemical oxidants kg NMVOC
6.87E-02 0 8.46E-04 3.44E-04 1.98E-03 -1.56E-02
(POCP) eq
Abiotic depletion potential for non fossil resources (ADPE) kg Sb eq 1.39E-04 0 3.33E-06 3.27E-07 1.83E-06 -8.37E-06
Abiotic depletion potential for fossil resources (ADPF) MJ 2.12E+02 0 1.98E+00 1.82E+00 1.24E+00 -6.84E+00
m3 world eq
Water use (WDP) 3.57E+00 0 7.1E-03 2.22E-02 -1.1E-01 -6.1E-02
deprived
RESULTS OF THE LCA - INDICATORS TO DESCRIBE RESOURCE USE according to EN 15804+A2: 1 m2 Veneered, wood
flooring with HDF carrier (10 mm) (10 mm)
Parameter Unit A1-A3 C1 C2 C3 C4 D
Renewable primary energy as energy carrier (PERE) MJ 2.86E+02 0 2.48E-02 2.23E-01 2.83E-02 -1.48E+02
Renewable primary energy resources as material utilization
MJ 0 0 0 0 0 0
(PERM)
Total use of renewable primary energy resources (PERT) MJ 2.86E+02 0 2.48E-02 2.23E-01 2.83E-02 -1.48E+02
Non renewable primary energy as energy carrier (PENRE) MJ 2.24E+02 0 2.11E+00 1.92E+00 1.35E+00 -7.27E+00
Non renewable primary energy as material utilization (PENRM) MJ 0 0 0 0 0 0
Total use of non renewable primary energy resources (PENRT) MJ 2.24E+02 0 2.11E+00 1.92E+00 1.35E+00 -7.27E+00
Use of secondary material (SM) kg 0 0 0 0 0 0
Use of renewable secondary fuels (RSF) MJ 0 0 0 0 0 0
Use of non renewable secondary fuels (NRSF) MJ 0 0 0 0 0 0
Use of net fresh water (FW) m3 1.23E-01 0 2.42E-04 1.08E-03 -2.07E-03 -1.82E-03
RESULTS OF THE LCA – WASTE CATEGORIES AND OUTPUT FLOWS according to EN 15804+A2:
1 m2 Veneered, wood flooring with HDF carrier (10 mm) (10 mm)
Parameter Unit A1-A3 C1 C2 C3 C4 D
Hazardous waste disposed (HWD) kg 2.3E-02 0 5.03E-06 7.44E-07 2.88E-06 -2.43E-05
Non hazardous waste disposed (NHWD) kg 3.52E+00 0 1.26E-01 1.22E-02 1.13E-01 -2.66E-01
Radioactive waste disposed (RWD) kg 9.65E-04 0 1.3E-05 7.01E-06 2.76E-06 -4.4E-05
Components for re-use (CRU) kg 0 0 0 0 0 0
Materials for recycling (MFR) kg 0 0 0 0 0 0
Materials for energy recovery (MER) kg 0 0 0 0 0 0
Exported electrical energy (EEE) MJ 0 0 0 0 2.45E+01 0
Exported thermal energy (EET) MJ 0 0 0 0 4.23E+01 0
RESULTS OF THE LCA – additional impact categories according to EN 15804+A2-optional:
1 m2 Veneered, wood flooring with HDF carrier (10 mm) (10 mm)
Parameter Unit A1-A3 C1 C2 C3 C4 D
Disease
Incidence of disease due to PM emissions (PM) 1.08E-06 0 1.18E-08 4.73E-09 1.66E-08 -2.51E-07
incidence
Human exposure efficiency relative to U235 (IR) kBq U235 eq 9.12E-01 0 8.31E-03 9.31E-03 2.04E-03 -2.87E-02
7 Environmental Product Declaration - Moland Group A/S - Moland Super Eg
Comparative toxic unit for ecosystems (ETP-fw) CTUe 3.76E+02 0 1.77E+00 2.37E+00 2.23E+00 -1.8E+02
Comparative toxic unit for humans (carcinogenic) (HTP-c) CTUh 2.34E-08 0 5.74E-11 4.83E-11 3.95E-10 -2.06E-09
Comparative toxic unit for humans (noncarcinogenic) (HTP-nc) CTUh 2.1E-07 0 1.93E-09 1.35E-09 2.1E-08 -7.51E-08
Soil quality index (SQP) SQP 1.5E+03 0 1.72E+00 3.27E-01 3.89E-01 -7.07E+02
Disclaimer 1 – for the indicator “Potential Human exposure efficiency relative to U235”. This impact category deals mainly with the
eventual impact of low-dose ionizing radiation on human health of the nuclear fuel cycle. It does not consider effects due to possible
nuclear accidents, occupational exposure or radioactive waste disposal in underground facilities. Potential ionizing radiation from the
soil, radon and from some construction materials is also not measured by this indicator.
Disclaimer 2 – for the indicators “abiotic depletion potential for non-fossil resources”, “abiotic depletion potential for fossil resources”,
“water (user) deprivation potential, deprivation-weighted water consumption”, “potential comparative toxic unit for ecosystems”,
“potential comparative toxic unit for humans – cancerogenic”, “Potential comparative toxic unit for humans - not cancerogenic”,
“potential soil quality index”. The results of this environmental impact indicator shall be used with care as the uncertainties on these
results are high as there is limited experience with the indicator.
6. LCA: Interpretation
parquet.
To visualize which materials and processes give the largest
contribution to the environmental indicators, a major The production of HDF gives the largest contribution to most of
contributions analysis has been included. In the graph, the total the environmental indicators. The exceptions are GWP where
value of each indicator has been set to 100 %. The colours the incineration of wood (waste) gives the largest contribution.
indicate which part of the environmental effects are caused by
the different materials and processes in the life cycle of the
7. Requisite evidence
Use phase (B) is not in the scope of this LCA, however, the Name Value Unit
emissions to indoor air will be mentioned informatively. VOC TVOC (C6 - C16) 6.1 μg/m3
emission test reports by Eurofins Product Testing A/S,
Sum SVOC (C16 - C22) < 5 μg/m3
Smedeskovvej 38, 8464 Galten, Denmark are available. The
highest measured values of all objects, included in group 3, is R (dimensionless) 0.092 -
given. VOC without NIK < 5 μg/m3
7.1. Formalehyde
Carcinogenic Substances < 1 μg/m3
Test method: EN 16516
Name Value Unit
EN 717-1 8.5 µg/m³
AgBB overview of results (3 days [µg/m³])
Name Value Unit
7.2. VOC emissions
TVOC (C6 - C16) 12 μg/m3
AgBB overview of results (28 days [µg/m³])
Sum SVOC (C16 - C22) < 5 μg/m3
R (dimensionless) 0.077 -
VOC without NIK < 5 μg/m3
Carcinogenic Substances < 1 μg/m3
8 Environmental Product Declaration - Moland Group A/S - Moland Super Eg
Name Value Unit
French VOC regulation A(+) -
Comparison with limit values of
French CMR components Pass -
- French VOC Regulation
Belgian Regulation Pass -
- French CMR Components
- Belgian Regulation
8. References
Standards ISO 21930
ISO 21930:2017 Sustainability in buildings and civil engineering
EN 322 works — Core rules for environmental product declarations of
EN 322:1994, Wood-based panels - Determination of moisture construction products and services, 2017.
content
Further references
EN 717-1
EN 717-1:5802004, Wood-based panels - Determination of AgBB/ABG
formaldehyde release - Part 1: Formaldehyde emission by the Anforderungen an bauliche Anlagen bezüglich des
chamber method Gesundheitsschutzes (ABG)
EN 12667 AltholzV
EN 12667:2001, Thermal performance of building materials and Ordinance on Requirements for the Recovery and Disposal of
products - Determination of thermal resistance by means of Waste Wood of 15 August 2002 (BGBl. I p. 3302), last
guarded hot plate and heat flow meter methods - Products of amended by Article 120 of the Ordinance of 19 June 2020
high and medium thermal resistance (BGBl. I p. 1328).
EN 13501-1 Belgian Regulation
EN 13501-1:2019, Fire classification of construction products Royal decree of May 2015
and building elements - Part 1: Classification using data from
reaction to fire tests BBSR
Bundesinstitut für Bau-, Stadt- und Raumforschung
ISO 14025
ISO 14025:2006 Environmental labels and declarations — Type BNB
III environmental declarations — Principles and procedures, BNB Code No. 352.812 Useful lives of building components for
2006. life cycle analyses according to the Sustainable Building
Assessment System, 2017: Wood multilayer parquet. Berlin:
ISO 14040 Federal Ministry of the Interior, for Construction and Home
ISO 14040:2006 Environmental management — Life cycle Affairs.
assessment — Principles and framework, 2006.
CDPH
ISO 14044 Californian Department of Public Health Standard Method for
ISO 14044:2006 Environmental management — Life cycle VOC Emissions
assessment — Requirements and guidelines, 2006.
ECHA Candidate List
EN 14342 List of Substances of Very High Concern (SVHC) Candidate for
EN 14342:2013, Wood flooring - Characteristics, evaluation of Authorisation (ECHA Candidate List), dated 17.01.2023,
conformity and marking published in accordance with Article 59(10) of the REACH
Regulation. Helsinki: European Chemicals Agency.
EN 14354
EN 14354: 2017, Wood veneer floor coverings EUROSTAT
European waste classification for statistics
CEN/TS 15676
CEN/TS 15676:2007, Wood flooring, slip resistance EWC-code
EWC-code 17 02 01: Non-hazardous wood waste
EN 15804
EN 15804:2012+A2:2019, Sustainability of construction works - French VOC Regulation
Environmental product declarations - Core rules for the product Regulation of March and May 2011 (DEVL1101903D and
category of construction products, 2019. DEVL1104875A)
EN 16485 French CMR Components
EN 16485:2014; Round and sawn timber - Environmental Regulation of April and May 2009
Product Declarations - Product category rules for wood and
wood-based products for use in construction, 2014. FSC®
Forest Stewardship Council License number: FSC-C095327
EN 16516
EN 16516:2017+A1:2020, Construction products: Assessment IBU 2021
of release of dangerous substances - Determination of Institut Bauen und Umwelt e.V.: General Instructions for the
emissions into indoor air. EPD programme of Institut Bauen und Umwelt e.V., Version
2.0, Berlin: Institut Bauen und Umwelt e.V., 2021 HYPERLINK
"http://www.ibu-epd." www.ibu-epd.com
9 Environmental Product Declaration - Moland Group A/S - Moland Super Eg
PCR Part B
Indoor Air Comfort Gold® 'Product Category Rules for Building-Related Products and
Eurofins product certification Services Part B: Requirements on the EPD for Solid wood
products.'
M1 Institut Bauen und Umwelt e.V., 2021.
Finnish classification test for building materials
Regulation (EU) No 305/2011
PEFC of the European Parliament and of the Council of 9 March 2011
Programme for the Endorsement of Forest Certification laying down harmonised conditions for the marketing of
Schemes. construction products
License number: PEFC/07-31-60
Regulation (EU) No 528/2012
PCR Part A of the European Parliament and the Council of 12 May 2012
'Product Category Rules for Building-Related Products and concerning the making available on the market and use of
Services Part A: Calculation Rules for the Life Cycle biocidal products.
Assessment and Requirements on the Project Report according
to EN 15804+A2:2019 Version 1.3,' Software/database
Ecoinvent database v3.6
10 Environmental Product Declaration - Moland Group A/S - Moland Super Eg
Publisher
Institut Bauen und Umwelt e.V. +49 (0)30 3087748- 0
Hegelplatz 1 info@ibu-epd.com
10117 Berlin www.ibu-epd.com
Germany
Programme holder
Institut Bauen und Umwelt e.V. +49 (0)30 3087748- 0
Hegelplatz 1 info@ibu-epd.com
10117 Berlin www.ibu-epd.com
Germany
Author of the Life Cycle Assessment
SGS INTRON +31 88 214 52 04
Dr. Nolenslaan 126 nl.intron@sgs.com
6136GV Sittard www.sgs.com/intron
Netherlands
Owner of the Declaration
Moland Group A/S +45 9614 5000
Strandvejen 16 moland@moland.dk
7800 Skive https://www.moland.dk/
Denmark
11 Environmental Product Declaration - Moland Group A/S - Moland Super Eg
