Environmental Product
Declaration
as per ISO 14025 and EN 15804
Owner of the declaration: Bitus Latvia SIA
Publisher: Kiwa-Ecobility Experts
Programme operator: Kiwa-Ecobility Experts
Declaration number: EPD-Kiwa-EE-000127-EN (Rev.1_30.05.2024)
Issue date: 04.05.2021
Valid to: 03.05.2026
Balcony doors and entrance
doors outward / inward opened
65 mm sash
(BYKO – DA65)
1. General information
Bitus Latvia SIA BYKO – DA65
Programme operator Owner of the declaration
Kiwa-Ecobility Experts Bitus Latvia SIA
Kiwa GmbH, Ecobility Experts Lāčplēša iela 75-5/6
Wattstraße 11-13 Rīga, LV-1011
13355 Berlin Latvia
Germany
Declaration number Declared product / declared unit
EPD-Kiwa-EE-000127-EN (Rev.1_30.05.2024) 1 m2 of product
This declaration is based on the Product Scope
Category Rules “Balcony door and entrance doors, outward /
Product category rules for windows and pe- inward opened, 65 mm sash” (BYKO-DA65) is
destrian doorsets (EN 17213) double-glazed and has a thermal transmit-
tance of 1,4 W/(m2*K). The dimensions height
Issue date x width) are made according to the customer's
04.05.2021 requirements. The calculation based on the
assumption of The LCA results are scalable for
Valid to the desired door dimension. The product is
03.05.2026 manufactured in Valmiera, Latvia, and mar-
keted internationally.
Kiwa-Ecobility Experts assumes no liability for
manufacturer's information, LCA data and ev-
idence.
Verification
The European standard EN15804:2020-03
serves as the core PCR
Independent verification of the declaration
and data according to ISO 14025:2011-10
☐internal ☒external
Raoul Mancke
(Head of programme operations, Kiwa-Ecobility Experts)
Martin Koehrer Joanna Zhuravlova, Ecomatters B.V.
(Verification body, Kiwa-Ecobility Experts) (Third party verifier)
Page | 2 Bitus Latvia SIA — BYKO-DA65
2. Product
2.1 Product description
All hardware is screwed in the sashes and frames. Door can be side opened. The dimensions (height x
width) are adapted according to customer requirements.
2.2 Application
The intended uses are in domestic and commercial locations.
2.3 Technical Data
For the description of the declared performances ((EU) No 305/2011) is used. The harmonized stand-
ard for windows and doors is EN 14351-1.
Characteristic Value Unit
Glass type Flat glass, double glazing -
Total weight* 43,9 kg
Thickness 65 mm
Glass surface* 0,58 m2
Heat permeability, door (U -value)
w 1,4 W/(m2*K)
(EN 10077)
Safety equipment n.a. -
Sound insulation n.a. db
Air permeability (EN 1026) n.a. -
Water tightness (EN12208) n.a. -
Resistance to wind load (EN 12210) Class C5 -
Racking (EN 14608) n.a. -
Torsion (EN 14609) n.a. -
Dangerous substances n.a.
* Reference size 1m2
Page | 3 Bitus Latvia SIA — BYKO-DA65
2.4 Placing on the market/ Application rules
For quality assurance purposes, windows and doors are regulated according to EN13249 . and marked
with a CE mark by the manufacturer. For the placing on the market the regulation (EU) No. 305/2011
and the performance characteristics EN 14351-1 apply.
2.5 Base materials / Ancillary materials
Raw material Value Unit
Wood 24,044 kg
Glass 14,503 kg
Steel 0,833 kg
Aluminium 2,047 kg
Plastics (TPE) 0,062 kg
Paint, impregnant, primer 2,286 kg
Argon 0,014 kg
2.6 Information on biogenic carbon content
Name Value Unit
Product 39,36 kg C
Packaging 1,75 kg C
2.7 Reference service life (RSL)
According the PCR B, no RSL must or can be indicated, since not all modules B1-B5 are declared.
2.8 Manufacture
The production phase (A3) consider the following processes: cutting of wood, preplanning, mould-ing
and tapening, chiseling, wood frame impregnation, assembly of wood components, painting, assembly
of glass and hardware, packaging. See also simplified process flowchart (figure 1).
2.9 Packaging
The door is wrapped in PE film and transported on wooden pallets.
Page | 4 Bitus Latvia SIA — BYKO-DA65
Figure 1: Simplified process flow chart of the manufacturing
Page | 5 Bitus Latvia SIA — BYKO-DA65
3. LCA: Calculation rules
3.1 Declared unit
In accordance with PCR B (EN 17213), one square metre was chosen as the declared unit for this door.
Further information for describing the declared unit be found in the tables below.
Description Value Unit
Declared unit 1 m2
Frame: Material type Redwood / Orgeno Pine (Douglas) -
Frame: Mass 11,925 / 12,119 kg
Glass: Material type Flat glass, double glazing, -
Glass: Mass 14,503 kg
Seal: Material type TPE / PU / PP / PE -
Seal: Mass 0,062 kg
Hardware: Material type Steel / Aluminium -
Hardware: Mass 0,620 / 2,481 kg
Total Mass 43,935 kg
Configuration 4-20-3/3 -
Gas type Argon -
Conversion factor to 1 kg 0,0228 m2/kg
3.2 System boundary
This Life cycle assessment is made for EPD type "Cradle to gate with modules C1-C4 and module D":
The Environmental Product Declaration analyses the production stage (A1-A3), the End-of-Life stage
(C1-C4) and the benefits and loads beyond the system boundary (D).
The door manufacturing process, the individual components such as framing materials or profiles,
hardware, glass, seals are delivered to the manufacturing site.
The processes that are performed at the manufacturing site are: Shaping of profiles, e.g. grinding of
wooden profiles, cutting extruded profiles into size (aluminium, etc.), assemble profiles, treatment and
coating of profiles and finally combining the infill and hardware with the profiles into a complete ele-
ment. C1 concerns the removal of the door, whereby no environmental impact is assumed. The result-
ing waste materials and quantities are included in the respective modules.
3.3 Estimates and assumptions
All installed raw materials of the products were analysed and the masses were determined. Produc-
tion-specific energy consumption were measured and provided by Bitus Latvia SIA. Supplier Infor-
mation regarding the transport distances were provided by Bitus Latvia SIA.
The production waste wood, metal and paint and other mixed production waste are collected sepa-
rately. For plastics and steel, 100 per cent recycling is assumed, and for general production waste, 100
per cent landfilling is assumed, as waste incineration is not widespread in Latvia. Wood waste is ther-
mally recovered at the site. For production waste that cannot be clearly allocated (seals, glass), a raw
material-related production reject of 5 percent was calculated. As the product is marketed interna-
tionally, no country-specific waste scenario can be considered. Therefore, the waste scenario of PCR B
(Appendix B.3) was adopted. Removing the door or window does not result in any environmental im-
pacts, so the value for module C1 is assumed to be zero.
Page | 6 Bitus Latvia SIA — BYKO-DA65
3.4 Cut-off criteria
For process modules A1 to A3, all process-specific data was collected. All flows could be assigned po-
tential environmental impacts through the Ecoinvent database. All flows that contribute more than
1 percent of the total mass, energy or environmental impact of the system have been included in the
LCA. The sum of neglect-ed processes does not exceed the 5 percent of total input mass for module
A1-A3.
The following in- and outputs were neglected: Infrastructure of the manufacturing, production waste
and municipal waste (except of wood, plastic, glass, waste water), lubricants and other ancillary mate-
rials.
3.5 Period under review
All process-specific data was collected for the operating year 2019.
3.6 Data quality
All process-specific data was collected for the 2019 operating year and is therefore up-to-date. The
data is based on the annual average. In order to ensure comparability of the results, only consistent
background data of the Ecoinvent database V3.5 was used in the LCA (e.g., records on energy, trans-
portation, supplies and supplies), which refers to reference year 2018. The database is regularly re-
viewed and thus complies with the requirements of EN 15804 (background data not older than 10
years). All consistent datasets contained in the Ecoinvent database are documented and can be viewed
in the online Ecoinvent documentation. The primary data were provided by Bitus Latvia SIA. The life
cycle was modelled with the Nibe EPD App. Geographical reference space of the background data is
Latvia. The overall representativeness and the precision for all datasets were determinate with the
Data Quality Ranking (DQR) formula, a ranking method based on the Product Environmental Footprint
(PEF) approach.
3.7 Allocation
There are no co-products in the raw material supply phase, so no allocation methods were used at this
stage. There are no allocations during the manufacturing phase at the plant.
3.8 Comparability
In principle, a comparison or evaluation of EPD data is only possible if all data sets to be compared
have been created in accordance with EN 15804 and the building context or the product-specific
performance characteristics have been taken into account.
Page | 7 Bitus Latvia SIA — BYKO-DA65
4. LCA: Results
The following tables show the results of the impact assessment indicators, resource use, waste and
other output streams. The results presented here refer to the declared average product.
Description of the system boundary
Benefits and
Construction loads beyond
Product stage Use stage End of life stage
process stage the system
boundaries
y lp p u s la ir e wt a am R t r o p s n a r T g n ir u t c a fu n a M u n a m m o r f t r o p s n a r T-e s u fo e c a lp o t r e r u t c a f n on io t cit ua rl tl sa nts on C-is s e c o r p e s U e c n a n e tn ia M r ia p e R tn e m e c a lp e R n e m h s ib r u fe R e s u y g r e n e la n o it a r e p O e s u r e t a w la n o it a r e p O / n o it c u r ts n eo Dc -n o itilo m e d t r o p s n a r T g n is s e c o r p e ts a W la s o p s iD y r e v eo s uc ee RR -- ga ni it ln c ye ct o e Rp -l
A1 A2 A3 A4 A5 B1 B2 B3 B4 B5 B6 B7 C1 C2 C3 C4 D
X X X MND MND MND MND MND MND MND MND MND X X X X X
X=Module declared | MND=Module not declared
Results of the LCA – Environmental impact: 1 m2 door - 65 mm sash (BYKO-D65)
Parameter Unit A1 A2 A3 C1 C2 C3 C4 D Total
Core environmental impact indicators (EN 15804)
ADP-f MJ 8,57E+02 6,43E+01 2,48E+02 0,00E+00 1,08E+01 2,76E+00 1,88E+00 -4,27E+02 7,58E+02
ADP-e kg Sb-eqv. 4,23E-04 1,17E-05 1,95E-05 0,00E+00 1,97E-06 6,57E-07 6,83E-08 -1,28E-04 3,29E-04
AP mol H+ eqv. 6,01E-01 2,37E-02 1,26E-01 0,00E+00 3,98E-03 8,06E-03 5,91E-04 -3,33E-01 4,31E-01
EP-fw kg PO4 eqv. 6,17E-03 6,22E-05 4,91E-04 0,00E+00 1,05E-05 1,08E-05 1,19E-06 -1,79E-03 4,96E-03
EP-m kg N eqv. 9,42E-02 8,31E-03 1,84E-02 0,00E+00 1,40E-03 3,70E-03 2,42E-04 -5,59E-02 7,04E-02
EP-t mol N eqv. 1,09E+00 9,20E-02 2,87E-01 0,00E+00 1,55E-02 4,24E-02 2,28E-03 -7,09E-01 8,23E-01
GWP-b kg CO2 eqv. -7,15E+01 1,20E-03 -6,25E+00 0,00E+00 2,02E-04 3,66E+01 1,31E-01 2,73E-02 -4,10E+01
GWP-f kg CO2 eqv. 7,84E+01 4,14E+00 1,59E+01 0,00E+00 6,96E-01 4,22E-01 6,51E-02 -4,66E+01 5,30E+01
GWP-luluc kg CO2 eqv. 1,06E+00 1,23E-03 8,63E-02 0,00E+00 2,07E-04 8,63E-05 1,75E-05 -1,87E-01 9,59E-01
GWP-total kg CO2 eqv. 7,95E+00 4,15E+00 9,72E+00 0,00E+00 6,97E-01 3,70E+01 1,97E-01 -4,68E+01 1,29E+01
ODP kg CFC 11 eqv. 4,99E-06 9,64E-07 2,54E-06 0,00E+00 1,62E-07 3,63E-08 2,71E-08 -1,77E-06 6,95E-06
POCP kg NMVOC eqv. 3,03E-01 2,62E-02 5,61E-02 0,00E+00 4,40E-03 1,11E-02 6,82E-04 -1,79E-01 2,22E-01
WDP m3 world eqv. 1,74E+01 4,57E-01 3,37E+00 0,00E+00 7,68E-02 1,15E+00 2,35E-02 -7,42E+00 1,50E+01
Additional environmental impact indicators (EN 15804)
ETP-fw CTUe 2,27E+03 4,61E+01 1,62E+02 0,00E+00 7,75E+00 2,27E+01 7,79E+01 -1,58E+03 1,01E+03
HTTP-c CTUh 1,01E-07 1,75E-09 1,35E-08 0,00E+00 2,94E-10 7,53E-09 2,89E-11 -6,27E-08 6,16E-08
HTTP-nc CTUh 1,98E-06 5,87E-08 1,37E-07 0,00E+00 9,86E-09 2,43E-08 8,89E-10 -1,19E-06 1,02E-06
IR kBq U235 eqv. 2,24E+00 2,73E-01 1,22E+00 0,00E+00 4,59E-02 8,39E-03 8,07E-03 -6,56E-01 3,14E+00
PM disease incidence 7,23E-06 3,76E-07 1,16E-06 0,00E+00 6,32E-08 6,58E-08 1,19E-08 -3,93E-06 4,98E-06
SQP - 6,57E+03 5,35E+01 8,57E+02 0,00E+00 9,00E+00 1,01E+00 3,96E+00 -1,90E+03 5,60E+03
ADP-e=Depletion of abiotic resources-elements | ADP-f=Depletion of abiotic resources-fossil fuels | AP=Acidification of soil and water |
EP-fw =Eutrophication, freshwater (EP-fw) | EP-m=Eutrophication marine (EP-m) | EP-T=Eutrophication, terrestrial (EP-T) | | GWP-
b=Global warming potential - Biogenic (GWP-b) | GWP-f=Global warming potential - Fossil (GWP-f) | GWP-luluc=Global warming potential
- Land use and land use change (GWP-luluc) |GWP-total=Global warming potential (GWP-total) |ODP=Ozone layer depletion |POCP=Pho-
tochemical oxidants creation | WDP=Water use (WDP) | ETP-fw=Ecotoxicity, freshwater | HTP-c=Human toxicity, cancer (HTP-c) | HTP-
nc=Human toxicity, non-cancer (HTP-nc) | IR=Ionising radiation, human health (IR) | PM=Particulate Matter (PM) | SQP=Land use (SQP)
Page | 8 Bitus Latvia SIA — BYKO-DA65
Resource use and environmental information: 1 m2 door - 65 mm sash (BYKO-D65)
Parameter Unit A1 A2 A3 C1 C2 C3 C4 D Total
PERE MJ 6,31E+02 6,73E-01 9,39E+01 0,00E+00 1,13E-01 1,25E-01 2,91E-02 -4,38E+02 2,87E+02
PERM MJ 3,36E+02 0,00E+00 3,96E+01 0,00E+00 0,00E+00 0,00E+00 0,00E+00 -3,46E-02 3,76E+02
PERT MJ 9,67E+02 6,73E-01 1,33E+02 0,00E+00 1,13E-01 1,25E-01 2,91E-02 -4,38E+02 6,63E+02
PENRE MJ 8,94E+02 6,82E+01 2,59E+02 0,00E+00 1,15E+01 2,97E+00 2,00E+00 -4,54E+02 7,84E+02
PENRM MJ 2,33E+01 0,00E+00 6,84E+00 0,00E+00 0,00E+00 0,00E+00 0,00E+00 0,00E+00 3,02E+01
PENRT MJ 9,17E+02 6,82E+01 2,66E+02 0,00E+00 1,15E+01 2,97E+00 2,00E+00 -4,54E+02 8,14E+02
SM Kg 3,06E-01 0,00E+00 3,06E-02 0,00E+00 0,00E+00 0,00E+00 0,00E+00 0,00E+00 3,37E-01
RSF MJ 0,00E+00 0,00E+00 0,00E+00 0,00E+00 0,00E+00 0,00E+00 0,00E+00 0,00E+00 0,00E+00
NRSF MJ 0,00E+00 0,00E+00 0,00E+00 0,00E+00 0,00E+00 0,00E+00 0,00E+00 0,00E+00 0,00E+00
FW m3 6,33E-01 1,21E-02 1,18E-01 0,00E+00 2,04E-03 1,24E-02 2,13E-03 -3,37E-01 4,43E-01
HWD Kg 1,43E-02 4,08E-05 1,58E-04 0,00E+00 6,86E-06 7,25E-06 8,56E-07 -2,33E-03 1,22E-02
NHWD Kg 1,30E+01 3,91E+00 2,24E+00 0,00E+00 6,57E-01 2,73E-01 1,16E+01 -7,50E+00 2,42E+01
RWD Kg 2,42E-03 4,32E-04 1,16E-03 0,00E+00 7,26E-05 9,71E-06 1,24E-05 -6,94E-04 3,42E-03
CRU Kg 0,00E+00 0,00E+00 0,00E+00 0,00E+00 0,00E+00 0,00E+00 0,00E+00 0,00E+00 0,00E+00
MFR Kg 0,00E+00 0,00E+00 2,93E-01 0,00E+00 0,00E+00 2,95E+00 0,00E+00 0,00E+00 3,24E+00
MER Kg 0,00E+00 0,00E+00 0,00E+00 0,00E+00 0,00E+00 0,00E+00 0,00E+00 0,00E+00 0,00E+00
EE MJ 0,00E+00 0,00E+00 1,94E+01 0,00E+00 0,00E+00 0,00E+00 0,00E+00 1,74E+02 1,93E+02
EET MJ 0,00E+00 0,00E+00 1,23E+01 0,00E+00 0,00E+00 0,00E+00 0,00E+00 1,10E+02 1,22E+02
EEE MJ 0,00E+00 0,00E+00 7,13E+00 0,00E+00 0,00E+00 0,00E+00 0,00E+00 6,39E+01 7,10E+01
PERE=renewable primary energy ex. raw materials | PERM=renewable primary energy used as raw materials | PERT=renewable primary
energy total | PENRE=non-renewable primary energy ex. raw materials | PENRM=non-renewable primary energy used as raw materials |
PENRT=non-renewable primary energy total | SM=use of secondary material | C= Carbon content | RSF=use of renewable secondary fuels
| NRSF=use of non-renewable secondary fuels | FW=use of net fresh water | HWD=hazardous waste disposed | NHWD=non-hazardous
waste disposed | RWD=radioactive waste disposed | CRU=Components for re-use | MFR=Materials for recycling | MER=Materials for energy
recovery | EE=Exported energy | EET=Exported Energy Thermic | EEE=Exported Energy Electric
Disclaimer on ADP-e, ADP-f, WDP, ETP-fw, HTP-c, HTP-nc, SQP: The results of these environmental
impact indicators must be used with caution, as the uncertainties in these results are high or as there
is limited experience with the indicator.
Disclaimer on IR: This impact category mainly addresses the potential effect of low dose ionizing radi-
ation on human health in the nuclear fuel cycle. It does not consider effects due to possible nuclear
accidents and occupational exposures, nor does it consider radioactive waste disposal in underground
facilities. Potential ionizing radiation from soil, radon, and some building materials is also not measured
by this indicator.
Page | 9 Bitus Latvia SIA — BYKO-DA65
5. LCA: Interpretation
5.1 Indicators of impact assessment by impact category
The following figure shows the influence of the different life stages. As shown in figure below, the raw
material (A1) and the manufacture (A3) have the greatest influence on the life cycle of BYKO-DA65. In
a further dominance analysis, the following inputs could be identified as drivers of environmental
impacts. Aluminium, glass, hardware. Potential credits come mainly from the material recovery of
aluminium. From the graph shown above, it can be deduced that, in principle, the module raw material
supply (A1) has the greatest influence on the life cycle assessment. For GWP biogenic, it is noticeable
that the sum is negative. Theoretically, the value should be close to zero in total, since the biogenic
carbon is released back into the atmosphere during incineration. This discrepancy is due to the fact
that the data sets do not match optimally. While in the wood products a 2,97 CO is stored by biomass
2
build-up, in the combustion process only a CO emission of 1,46 of kg wood is calculated. The packaging
2
material (wooden pallets) also contributes with a negative input, while the CO emission from com-
2
bustion is not included, as this is assigned to the undeclared module A5.
BYKO-DA65
100%
80%
D
60%
C4
40%
20% C3
0% C2
-20%
C1
-40%
A3
-60%
-80% A2
A1
Figure 2: Influence of the information modules on the main impact categories – BYKO-DA65
5.2 Information on data quality
The data quality can be classified as good overall. All relevant process-specific data could be collected
in the operational data collection. Consistent data sets from the Ecoinvent database were available for
almost all inputs and outputs. The background data meet the requirements of EN 15804, and the pro-
duction data were recorded for the 2019 operating year. The quantities of raw materials and supplies
used as well as energy consumption were recorded for the entire operating year. The life cycle as-
sessment was carried out for all the product items listed. It can be assumed that the data for the de-
clared average product are well representative.
Data quality was calculated using the Data Quality Rating method according to the PEF approach. The
DQRs range from 1,75 to 2,0 for the most abundant inputs in terms of mass, and from 2,0 to 2,5 for
smaller inputs. As noted in the interpretation (GWP biogenic), partial data sets are not entirely con-
sistent with each other.
Page | 10 Bitus Latvia SIA — BYKO-DA65
6. References
EN 14351-1:2016-12: Windows and doors - Product standard, performance characteristics - Part 1:
Windows and external pedestrian doorsets
EN 15804:2020: Sustainability of construction works — Environmental Product Declarations — Core
rules for the product category of construction products
EN 17213:2018: Windows and doors – Environmental Product Declarations – Product category rules
for windows and pedestrian doorsets
European Commission Joint Research Centre Institute for Prospective Technological Studies (JCR
2014): End-of-waste criteria for waste plastic for conversion, Seville, 2014, doi:10.2791/13033
CML-IA April 2013 – Charakterisierungsfaktoren entwickelt durch Institut of Environmental Sciences
(CML): Universität Leiden, Niederlande - http://www.cml.leiden.edu/software/data-cmlia.html
Klöpffer, W., Grahl B.: Ökobilanz (LCA) – Ein Leitfaden für die Ausbildung und Beruf, Wily-VCH Verlag,
Weinheim, 2007
ISO 14040:2006-10, Environmental management - Life cycle assessment - Principles and framework;
EN ISO 14040:2006
ISO 14044:2006, Environmental management - Life cycle assessment - Requirements and guidelines;
EN ISO 14040:2006
ISO 14025:2011-10: Environmental labels and declarations — Type III environmental declarations —
Principles and procedures EN 13249
Protocol EPD-online - 25011.16.03.015 - Protocol EPD online - NMD, version 1.2, November 2016, NIBE
Stichting Bouwkwaliteit (SBK 2019): Determination Method for determining the environmental perfor-
mance of buildings and civil engineering works over their entire service life, based on EN 15804, Rijs-
wijk, Version "3.0 January 2019" incl. amendments July 2019, Jan 2020
Stichting Bouwkwaliteit: verification protocol - inclusion data in the Dutch environmental database,
Rijswijk, Final Version 3.0, January 2019
Page | 11 Bitus Latvia SIA — BYKO-DA65
Publisher Mail DE.Ecobility.Ex-
Kiwa-Ecobility Experts perts@kiwa.com
Kiwa GmbH, Ecobility Experts Web https://www.kiwa.com/de/
Wattstraße 11-13 de/themes/ecobility-ex-
13355 Berlin perts/ecobility-experts/
Germany
Programme operator Mail DE.Ecobility.Ex-
Kiwa-Ecobility Experts perts@kiwa.com
Kiwa GmbH, Ecobility Experts Web https://www.kiwa.com/de/
Wattstraße 11-13 de/themes/ecobility-ex-
13355 Berlin perts/ecobility-experts/
Germany
LCA Practitioner
Kiwa GmbH, Ecobility Experts Tel. +49 30 467761 43
Wattstraße 11-13 Mail DE.Nachhaltigkeit@kiwa.com
13355 Berlin Web www.kiwa.com
Germany
Owner of the declaration Tel. +371 220 088 85
Bitus Latvia SIA Mail info@bitus.lv
Lāčplēša iela 75-5/6 Web https://bitus.com/latvia-
Rīga, LV-1011 ee/
Latvia
Page | 12 Bitus Latvia SIA — BYKO-DA65
