ENVIRONMENTAL PRODUCT DECLARATION
as per ISO 14025 and EN 15804+A2
Owner of the Declaration VELUX Group
Publisher Institut Bauen und Umwelt e.V. (IBU)
Programme holder Institut Bauen und Umwelt e.V. (IBU)
Declaration number EPD-VEL-20220142-IBJ3-EN
Issue date 25.07.2022
Valid to 24.07.2027
VELUX flat roof window CFU
VELUX A/S
www.ibu-epd.com | https://epd-online.com
1. General Information
VELUX A/S VELUX flat roof window CFU
Programme holder Owner of the declaration
IBU – Institut Bauen und Umwelt e.V. VELUX Group
Hegelplatz 1 Ådalsvej 99
10117 Berlin 2970 Hørsholm
Germany Denmark
Declaration number Declared product / declared unit
EPD-VEL-20220142-IBJ3-EN The declaration represents 1 piece of a VELUX flat roof window CFU with
a fixed base unit of the size 1.20 m x 1.20 m = 1.44 m2
This declaration is based on the product category rules: Scope:
Windows and doors , 01.08.2021 The declaration covers 100% of VELUX flat roof windows CFU with a fixed
(PCR checked and approved by the SVR) base unit by Østbirk Bygningsindustri, Denmark.
The owner of the declaration shall be liable for the underlying information
and evidence; the IBU shall not be liable with respect to manufacturer
Issue date information, life cycle assessment data and evidences.
25.07.2022
The EPD was created according to the specifications of EN 15804+A2. In
the following, the standard will be simplified as EN 15804.
Valid to
Verification
24.07.2027
The standard EN 15804 serves as the core PCR
Independent verification of the declaration and data according to ISO
14025:2011
internally X externally
Dipl.-Ing. Hans Peters
(Chairman of Institut Bauen und Umwelt e.V.)
Florian Pronold Dr. Eva Schmincke,
(Managing Director Institut Bauen und Umwelt e.V.) (Independent verifier)
1 Environmental Product Declaration - VELUX A/S - VELUX flat roof window CFU
2. Product
The product is available in pre-defined sizes covering 0,6x0,6m
2.1 Product description/Product definition to 1,5x1,5m.
The VELUX flat roof window CFU consists of a fixed base unit
made of a PUR/GRP curb with a wooden core, integrated 2.5 Base materials/Ancillary materials
glazing unit and a single layer flat or curved glass top unit on Composition of the base unit CFU:
top. For the placing of the product on the market in the
European Union/European Free Trade Association /EU/EFTA) polyurethane 8 %
(with the exception of Switzerland) the Regulation (EU) No.
305/2011 (CPR) applies. The product needs a declaration of heat-treated wood 10 %
performance taking into consideration EAD 220062-00-0401,
June 2017, rooflight with bonded or mechanically fastened aluminium 10 %
cover glass and the CE-marking. For the application and use
the respective national provisions apply. galvanized steel 5 %
2.2 Application PVC 3 %
Velux flat roof windows CVU are used in renovation and new
build. laminated glass 30 %
2.3 Technical Data
tempered glass 15 %
The Declaration of Performance including relevant technical
specifications and test methods/test standards can be heat strenghtened glass 15 %
downloaded from the website www.velux.com/ce.
others
The declared values in the table relate to the reference product
incl. an average pane. For other covered product variants, Composition of the top unit (ISU 1093):
specific values can be selected at the bottom of the above-
mentioned download page Curved glass 73 %
Constructional data for CFU 120120 20+ISU 1093
For other variants, see velux.com/ce Aluminium 25 %
Name Value Unit
others
External fire
performance EN NPD -
1) 'This product/article/at least one partial article contains
13501-5
substances listed in the candidate list (date: 02.03.2022)
Water tightness EN exceeding 0.1 percentage by mass:
9A Class
1873
• no
Resistance to wind
C3 Class 2) 'This product/article/at least one partial article contains other
load
CMR substances in categories 1A or 1B which are not on the
5 mm toughened/ -- / 4 mm candidate list, exceeding 0.1 percentage by mass:
Resistance to snow
toughened / 16 mm / 7.5 mm -
load • not investigated with suppliers
(33.4) laminated float
3) 'Biocide products were added to this construction product or
Impact resistance 3 Class it has been treated with biocide products (this then concerns a
Bonding of cover treated product as defined by the (EU) Regulation on Biocidal
Compliant (ΔX≥0.75) -
glass Products No. 528/2012):
Airborne sound • no
insulation EN ISO 39 (-1;-5) dB
410-3
Thermal Recycled content
Urc,ref300: 0,65 W/(m2K)
transmittance EN -
Arc,ref300: 4,4 m2
1873
Total solar energy
0,52 -
transmittance
Light transmittance
0,69 -
EN 410
Frame factor 0,1 -
Air permeability EN The values stated in the table relate to the recycled material
4 Class
1026 streams in VELUX production.
Performance data of the product in accordance with the
declaration of performance with respect to its essential
2.6 Manufacture
characteristics according to
Base unit:
• EAD 220062-00-0401, June 2017, rooflight with bonded
or mechanically fastened cover glass. The PU raw material, gaskets and other minor components are
produced outside Velux.
2.4 Delivery status
2 Environmental Product Declaration - VELUX A/S - VELUX flat roof window CFU
Cutting and profiling of wood reinforcements are done at
production sites in Polen and Denmark. Health protection: According to current knowledge, no health
hazards or impairments are to be expected.
The PUR/GRP curb with wooden core and the insulating glass
unit are assembled at the production site in Denmark. 2.12 Reference service life
It is not possible to calculate the reference service life
The production and final assembly of the base unit takes place according to ISO 15686. The service life based on a
at the production site in Denmark. manufacturer's declaration is 30 years. The corresponding
utilization scenario is declared in 4.
The final production processes include preparation of the
2.13 Extraordinary effects
PU/wood frame by cutting and profiling of wood, moulding,
cutting, sandblasting and painting, cutting and mounting of Fire
gaskets and installation of glazing unit as well as packaging,
stacking and wrapping of the product on pallets. Fire performance according to EN 13501:1
Name Value
Top unit:
Building material class D
All raw materials and components are produced outside Velux. Burning droplets s2
Smoke gas development d2
The glass top unit is assembled at the production site in
Slovakia.
Water
In the event of unforeseen exposure to water (flood), VELUX
The final production processes include assembly of product, as
flat roof windows must be replaced as electrical components;
well as packaging, stacking and wrapping of the product on
no adverse effects on human health or the environment are to
pallets. The factories are ISO 9001 certified.
be expected.
2.7 Environment and health during manufacturing
Mechanical destruction
All factories are ISO 14001 and ISO 45001 certified.
In the event of unforeseen mechanical destruction, VELUX flat
2.8 Product processing/Installation roof windows must be replaced; apart from potential injuries
from glass cullet, no adverse effects on human health or the
The product is delivered to the customer in two parts, a top and
environment are to be expected.
bottom part. After the hole in the roof is prepared, the bottom
part of the product can be installed with the use of a
2.14 Re-use phase
screwdriver, after which the top unit can be fastened to the
VELUX flat roof windows can be dismantled manually without
bottom unit.
any problems. The metal parts are usually recycled, and the
2.9 Packaging plastic parts and wood are sent for thermal recycling for energy
recovery. Flat glass can be recycled whereas laminated glass is
The packaging usually consists of:
usually used as secondary aggregate in road construction or
- polyethylene film
landfilling.
- polystyrene foam parts
- cardboard
2.15 Disposal
VELUX flat roof windows are mostly inert and can be disposed
The use of other packaging materials is possible, but
of in an appropriate landfill. However, due to the value of the
insignificant in terms of quantity.
materials or the carbon content of the plastic parts and wood,
recycling or energy recovery is preferable and common.
The plastic packaging (polyethylene (PE) film, polystyrene foam
parts) can be recycled if separated by type; alternatively, they
Waste code according to the European Waste List (Regulation
can be incinerated.
on the European Waste List):
2.10 Condition of use
17 02 01 wood
The material composition of VELUX flat roof windows does not
17 02 02 glass
change over their service life.
17 02 03 plastics
2.11 Environment and health during use 17 04 14 mixed metals
VELUX flat roof windows do not contain any pollutants that
2.16 Further information
could be released during use.
Further documentation on the products, technical data sheets,
BIM files, etc. can be found at:
Environmental protection: According to current knowledge,
www.velux.com
hazards to water, air and soil cannot arise when the products
are used as intended.
3. LCA: Calculation rules
Name Value Unit
3.1 Declared Unit
Declared unit 1 pce.
The declared unit is 1 piece of a fixed VELUX flat roof window
Area 1.44 m²
CFU with a base unit made of a polyurethane, heat-treated
wood and plywood with an integrated glazing unit with 1.20 m x Weight 133 kg
1.20 m = 1.44 m2.
Declared unit
3 Environmental Product Declaration - VELUX A/S - VELUX flat roof window CFU
No further assumptions and estimates relevant to the result had
3.2 System boundary to be made beyond the points made in this chapter 3 and in
Type of EPD: Cradle to gate with options, with modules C1 – chapter 4.
C4, and module D (A1-A3, C1-C3, D and additional modules
3.4 Cut-off criteria
The production of VELUX flat roof windows (modules A1-A3) No data available from the company survey was neglected.
includes raw material extraction, energy generation, waste These include, among other things, material use, energy
treatment and all transports up to the factory gate. In demand (heat, electricity), packaging materials of raw materials
accordance with COUNCIL REGULATION (EU) No 333/2011, (insofar as they are generated as waste) and product
secondary metals are modeled as part of the product system packaging, consumables in production, waste treatment and
from the moment they are available as unmixed scrap. the transport of all inputs and outputs.
Waste or secondary fuels are not used for production. With this approach, mass and energy flows below 1 % were
also accounted for. No processes were neglected that would
Module A4 is not declared due to large variances in transport have been known to the project managers and would have
distances between the production site and the construction site, contributed significantly to the indicators of the impact
where the product is installed. assessment.
Module A5: The products are delivered to the construction site 3.5 Background data
ready to be installed. Manual installation is assumed, and Ecoinvent 3.8 (2021) is used as the background database.
electricity consumption related to electric drilling machines,
3.6 Data quality
screw drivers, etc. is considered to be negligible. The
combustible packaging material (plastics, wood, etc.) is The foreground data are based on extensive and detailed data
assumed to be thermally treated in a municipal waste collection at the production site. The foreground data could be
incineration plant with an efficiency R1 < 0.6 (according to the fully linked with corresponding data records from the
ecoinvent dataset used); the recovered energy is declared as background database ecoinvent 3.8.
exported energy. Metals and cardboard are recycled; it is The background data was updated in 2021. Thus, the quality of
assumed that these fractions reach the end-of-waste state after the foreground and background data can be rated as very
having been sorted and transported (as a conservative choice) good.
to a recycler. No packaging waste is landfilled.
3.7 Period under review
The LCA data represents the production conditions for the year
Modules B1 to B7 are not relevant for the product under
2021.
consideration or no significant environmental impacts occur.
3.8 Geographic Representativeness
Module C1 includes manual dismantling, with no significant
Land or region, in which the declared product system is
environmental impact.
manufactured, used or handled at the end of the product´s
lifespan: Europe
Module C2 comprises the transport of the dismantled VELUX
flat roof window to a sorting plant and then to a waste
incineration plant for the thermally treated plastic fraction. 3.9 Allocation
No co-products are generated during the production of the
Modules C3/C4: given the complexity of the inventoried VELUX products. Sorted production scrap of the different
products, a mixed end-of-life scenario is modelled, allowing the metals, notably aluminium, is considered a secondary material
different materials to follow their most likely path. with no economic value (so no burdens allocated) and
As a rule of thumb, metals are recycled and plastics are considered in the quantification of net flows leaving the product
incinerated (also due to the very limited data availability of system. This approach is chosen to ensure a coherent
plastics recycling and its benefits); coated and uncoated flat quantification of net flows entering module D.
glass is assumed to be recycled whereas laminated glass is Biogenic carbon is allocated based on physical flows
assumed to be landfilled due to very limited recycling potential. regardless of the allocation procedure chosen for the process.
Metals and flat glass recycled; it is assumed that these fractions The biogenic carbon content of wood products entering or
reach the end-of-waste state after having been sorted and leaving the product system is quantified (manually) as part of
transported to a recycler; laminated glass is landfilled. The the GWP in conformity with DIN EN 16485.
combustible material (plastics, wood, etc.) is assumed to be
thermally treated in a municipal waste incineration plant. No processes were modelled as part of the foreground model
that would have required an allocation of multi-input processes.
Module D includes the benefits and burdens associated with Background datasets on municipal waste incineration plants
recycling metals beyond the system boundary, resulting from were taken from ecoinvent without any modification.
the treatment of recycled materials from the point of end-of-
waste to the point of substitution (as loads) and substitution of Allocation of reuse, recycling and recovery was avoided by the
primary resources (as benefits). cut-off approach in the foreground model in line with DIN EN
It also includes the benefits and burdens associated with 15804.
energy recovery from plastic waste in a municipal waste
incineration plant, as modeled in Module C3. 3.10 Comparability
In Module D, only net flows of metals leaving the product Basically, a comparison or an evaluation of EPD data is only
system are considered. possible if all the data sets to be compared were created
according to EN 15804 and the building context, respectively
3.3 Estimates and assumptions
the product-specific characteristics of performance, are taken
into account.
4. LCA: Scenarios and additional technical information
4 Environmental Product Declaration - VELUX A/S - VELUX flat roof window CFU
Name Value Unit
Characteristic product properties of biogenic carbon
Reference service life
according to 30 a
Information on describing the biogenic carbon content at manufacturer's declaration
factury gate The product has passed
Declared product
Name ValueUnit internal quality controls and
properties (at the gate) and -
kg complies with EAD 220062-
Biogenic carbon content in product 4.57 finishes
C 00-0401 for CE marking
Biogenic carbon content in accompanying kg Design application
2.22
packaging C parameters (if instructed by
Installation according to
the manufacturer),
Note: 1 kg of biogenic carbon is equivalent to 44/12 kg of CO . assembly instructions and -
2 including the references to
state of the art.
the appropriate practices
and application codes
An assumed quality of
Carried out in accordance
work, when installed in
with the manufacturer's -
accordance with the
Module A5 instructions.
manufacturer’s instructions
The products are delivered to the construction site ready to be
Outdoor environment, (for The declared products are
installed. Manual installation is assumed, and electricity
outdoor applications), e.g. intended for installation
consumption related to electric drilling machines, screw drivers,
weathering, pollutants, UV outside the building: They are
etc. is considered to be negligible. -
and wind exposure, therefore designed to
building orientation, withstand outdoor conditions
The combustible packaging material (plastics, wood, etc.) is
shading, temperature throughout their service life.
assumed to be transported 50 km with a lorry 16-32 metric
tons, EURO6 to an incineration plant with an efficiency R1 < 0.6 Indoor environment (for
The declared products are
(according to the ecoinvent dataset used); the recovered indoor applications), e.g.
not intended for installation -
energy is declared as exported energy; for its quantification an temperature, moisture,
inside a building.
efficiency of 25.6 % is assumed for the production of heat and chemical exposure
13.0 % for the production of electricity (always referring to the Usage conditions, e.g. Standard use in any type of
lower heating value of the waste). frequency of use, building, i.e. opening/closing -
mechanical exposure as often as necessary.
Metals and cardboard are recycled; it is assumed that these The declared products are
fractions reach the end-of-waste state after having been sorted Maintenance e.g. required designed for a reference life
and transported (as a conservative choice) to a recycler over frequency, type and quality of 30 years. They are
-
150 km with a lorry 16-32 metric tons, EURO6. and replacement of maintained by cleaning water
components at the discretion of the
No packaging waste is landfilled. building occupants.
Module B1
The use of multi-way pallets is not taken into account as
The products are assumed to have no direct emissions during
packaging material.
the use phase. The indicator values of Module B1 are thus 0.
For biogenic carbon stored in product, see above.
Reference service life
Module B2
Annual cleaning with water (e.g., using 1 l/m2 of tap water per
annual cleaning) is neglected.
Module B6
No electricity is used.
Module C1
Manual de-installation is assumed, electricity consumption
related to electric screw drivers, etc. is considered to be
negligible. Thus, no environmental impacts are declared in
module C1.
Module C2
Given the complexity of the inventoried products, a mixed end-
of-life scenario is modelled, allowing the different materials to
follow their most likely path.
It should also be noted that the deconstruction and waste
treatment scenario can vary a lot, depending on the actual
situation. Thus, a generic end-of-life scenario is assumed.
As a rule of thumb, metals are recycled, plastics are incinerated
(also due to the very limited availability on plastics recycling
and its benefits); coated and uncoated flat glass is assumed to
5 Environmental Product Declaration - VELUX A/S - VELUX flat roof window CFU
be recycled whereas laminated glass is assumed to be
landfilled due to very limited recycling potential. Some of the material, notably laminated flat glass is assumed
to be landfilled.
The combustible material (plastics, wood, etc.) is assumed to
be transported 50 km with a lorry 16-32 metric tons, EURO6 to Module D
an incineration plant. Module D contains the benefits and loads beyond the system
boundary related to the recycling of metals, which result from
Metals and flat glass recycled; it is assumed that these fractions the treatment of recycled materials from the point of end-of-
the each end-of-waste state after having been sorted and waste status to the point of substitution (as loads) and the
transported to a recycler over 150 km with a lorry 16-32 metric substitution of primary resources (as benefits).
tons, EURO6.
Furthermore, it includes the benefits of raw material substitution
Laminated glass is landfilled, including a transport of 30 km with of the recycling of flat glass, with the exception of laminated
a lorry 16-32 metric tons, EURO6. glass, which cannot be used for the production of glass again.
Recovered flat glass is assumed to have reached the end-of-
Module C3 waste state as sorted glass cullet; glass cullet is assumed to
A consumption of 0.03 kWh/kg of electricity for shredding and replace virgin raw material for glass production – impacts on
sorting and 0.437 MJ/kg of diesel fuel for internal logistics are the energy required to remelt recycled glass as compared to
taken into account to disassemble the product. The recovered virgin glass production are neglected due to a lack of data.
material leaves the product system as 'materials for recycling'.
The net amounts of the metals leaving the product system are It also includes the benefits and loads related to the energy
considered as 'use of secondary material' in Module D. recovery from plastic wastes in a MWIP as modelled in
Modules A3, A5 and C3.
Module C4
As stated above, it is assumed that 100 % of the plastic parts Due to a lack of data for plastics from de-construction activities,
and the wooden parts are treated in a waste incineration plant the substitution potential of recycled plastics is not taken into
with an efficiency R1 < 0.6 (according to the ecoinvent dataset account.
used); 25.57 % of the lower heating value of the plastic parts
are recovered as heat and 13.0 % as electricity. Recovered Only net flows leaving the product system are considered in
energy is reported as 'exported energy' and considered in module D.
Module D.
6 Environmental Product Declaration - VELUX A/S - VELUX flat roof window CFU
5. LCA: Results
Disclaimer:
EP-freshwater: This indicator has been calculated as 'kg P eq' as required in the characterization model (EUTREND model, Struijs et
al., 2009b, as implemented in ReCiPe; http://eplca.jrc.ec.europa.eu/LCDN/developerEF.xhtml)
DESCRIPTION OF THE SYSTEM BOUNDARY (X = INCLUDED IN LCA; MND = MODULE OR INDICATOR NOT DECLARED; MNR
= MODULE NOT RELEVANT)
Benefits and
Construction loads beyond
Product stage Use stage End of life stage
process stage the system
boundaries
la ire ta m w a Ry lp p u s tro p s n a rT g n iru tc a fu n a M e h t m o rf tro p s n a rTe tis e h t o t e ta g y lb m e s s A e s U e c n a n e tn ia M ria p e R tn e m e c a lp e R tn e m h s ib ru fe R y g re n e la n o ita re p Oe s u re ta w la n o ita re p Oe s u n o itc u rts n o c -e Dn o itilo m e d tro p s n a rT g n is s e c o rp e ts a W la s o p s iD -e s u e R-y re v o c e R-g n ilc y c e Rla itn e to p
A1 A2 A3 A4 A5 B1 B2 B3 B4 B5 B6 B7 C1 C2 C3 C4 D
X X X MND X X X MNR MNR MNR X MND X X X X X
RESULTS OF THE LCA - ENVIRONMENTAL IMPACT according to EN 15804+A2: 1 piece fixed VELUX flat roof window CFU,
1.20 m x 1.20 m = 1.44 m2
Parameter Unit A1-A3 A5 B1 B2 B6 C1 C2 C3 C4 D
GWP-total kg CO 2 eq 5.18E+02 2.1E+01 0 0 0 0 1.31E+00 1.55E+00 5.65E+01 -3.39E+02
GWP-fossil kg CO 2 eq 5.5E+02 5.19E+00 0 0 0 0 1.31E+00 1.54E+00 3.97E+01 -3.38E+02
GWP-
biogenic kg CO 2 eq -3.25E+01 1.58E+01 0 0 0 0 0 6.56E-03 1.67E+01 0
GWP-luluc kg CO 2 eq 9.6E-01 1.89E-04 0 0 0 0 5.35E-04 1.71E-03 3.29E-03 -1.17E+00
ODP kg CFC11 eq 6.81E-05 1.07E-07 0 0 0 0 3.08E-07 9.48E-08 1.22E-06 -1.26E-05
AP mol H+ eq 2.74E+00 3.04E-03 0 0 0 0 7.45E-03 5.88E-03 3.29E-02 -2.04E+00
EP-
kg P eq 1.5E-02 3.66E-06 0 0 0 0 9.66E-06 1.99E-04 9.91E-05 -1.39E-02
freshwater
EP-marine kg N eq 5.01E-01 1.15E-03 0 0 0 0 2.68E-03 1.88E-03 1.37E-02 -3.05E-01
EP-terrestrial mol N eq 5.27E+00 1.27E-02 0 0 0 0 2.95E-02 2.14E-02 1.42E-01 -3.37E+00
kg NMVOC
POCP 1.54E+00 3.57E-03 0 0 0 0 8.42E-03 5.71E-03 3.47E-02 -9.96E-01
eq
ADPE kg Sb eq 8.98E+02 1.57E-06 0 0 0 0 4.4E-06 2.68E-06 2.66E-05 2.68E-03
ADPF MJ 5.02E+03 7E+00 0 0 0 0 2.02E+01 2.12E+01 3.48E+01 -3.23E+03
m3 world eq
WDP 1.32E+02 2.93E-02 0 0 0 0 6.64E-02 5.29E-02 1.92E+00 -4.23E+01
deprived
GWP = Global warming potential; ODP = Depletion potential of the stratospheric ozone layer; AP = Acidification potential of land and water; EP =
Eutrophication potential; POCP = Formation potential of tropospheric ozone photochemical oxidants; ADPE = Abiotic depletion potential for non-fossil
resources; ADPF = Abiotic depletion potential for fossil resources; WDP = Water (user) deprivation potential)
RESULTS OF THE LCA - INDICATORS TO DESCRIBE RESOURCE USE according to EN 15804+A2: 1 piece fixed VELUX flat
roof window CFU, 1.20 m x 1.20 m = 1.44 m2
Parameter Unit A1-A3 A5 B1 B2 B6 C1 C2 C3 C4 D
PERE MJ 4.32E+02 1.08E-01 0 0 0 0 2.86E-01 2.69E+00 1.82E+02 -4.07E+02
PERM MJ 3.6E+02 -1.81E+02 0 0 0 0 0 -8.46E-02 -1.79E+02 0
PERT MJ 7.92E+02 -1.81E+02 0 0 0 0 2.86E-01 2.6E+00 2.95E+00 -4.07E+02
PENRE MJ 6.2E+03 6.77E+01 0 0 0 0 2.02E+01 1.7E-05 4.31E+02 -3.24E+03
PENRM MJ 4.57E+02 -6.07E+01 0 0 0 0 0 0 -3.97E+02 0
PENRT MJ 6.66E+03 7E+00 0 0 0 0 2.02E+01 1.7E-05 3.48E+01 -3.24E+03
SM kg 2.23E+01 0 0 0 0 0 0 0 0 4.32E+00
RSF MJ 0 0 0 0 0 0 0 0 0 0
NRSF MJ 0 0 0 0 0 0 0 0 0 0
FW m3 4.17E+00 1.53E-03 0 0 0 0 2.2E-03 5.07E-03 5.95E-02 -2.11E+00
PERE = Use of renewable primary energy excluding renewable primary energy resources used as raw materials; PERM = Use of renewable primary
energy resources used as raw materials; PERT = Total use of renewable primary energy resources; PENRE = Use of non-renewable primary energy
excluding non-renewable primary energy resources used as raw materials; PENRM = Use of non-renewable primary energy resources used as raw
materials; PENRT = Total use of non-renewable primary energy resources; SM = Use of secondary material; RSF = Use of renewable secondary fuels;
NRSF = Use of non-renewable secondary fuels; FW = Use of net fresh water
RESULTS OF THE LCA – WASTE CATEGORIES AND OUTPUT FLOWS according to EN 15804+A2:
1 piece fixed VELUX flat roof window CFU, 1.20 m x 1.20 m = 1.44 m2
Parameter Unit A1-A3 A5 B1 B2 B6 C1 C2 C3 C4 D
HWD kg 6.99E-02 1.9E-05 0 0 0 0 5.16E-05 1.7E-05 6.86E-05 4.04E-02
NHWD kg 1.06E+02 5.3E-01 0 0 0 0 1.36E+00 8.65E-02 5.03E+01 -7.58E+01
7 Environmental Product Declaration - VELUX A/S - VELUX flat roof window CFU
RWD kg 4.63E-02 9.92E-05 0 0 0 0 2.92E-04 1.92E-04 2.88E-04 -1.05E-02
CRU kg 0 0 0 0 0 0 0 0 0 0
MFR kg 4.09E+00 1.07E+01 0 0 0 0 0 4.82E+01 0 0
MER kg 0 0 0 0 0 0 0 0 0 0
EEE MJ 1.52E+01 7.89E+00 0 0 0 0 0 0 7.48E+01 0
EET MJ 2.95E+01 1.55E+01 0 0 0 0 0 0 1.47E+02 0
HWD = Hazardous waste disposed; NHWD = Non-hazardous waste disposed; RWD = Radioactive waste disposed; CRU = Components for re-use;
MFR = Materials for recycling; MER = Materials for energy recovery; EEE = Exported electrical energy; EET = Exported thermal energy
RESULTS OF THE LCA – additional impact categories according to EN 15804+A2-optional:
1 piece fixed VELUX flat roof window CFU, 1.20 m x 1.20 m = 1.44 m2
Parameter Unit A1-A3 A5 B1 B2 B6 C1 C2 C3 C4 D
Disease
PM 2.78E-05 4.37E-08 0 0 0 0 1.18E-07 9.13E-08 2.17E-07 -2.4E-05
incidence
IR kBq U235 eq 1.03E+01 3E-02 0 0 0 0 8.78E-02 7.38E-02 1.38E-01 -3.99E+00
ETP-fw CTUe 1.18E+04 2.66E+01 0 0 0 0 1.6E+01 1.25E+01 4.77E+02 -6.45E+03
HTP-c CTUh 9.81E-07 9.01E-10 0 0 0 0 6.39E-10 3.38E-10 1.15E-08 -3.39E-07
HTP-nc CTUh 1.3E-05 1.21E-08 0 0 0 0 1.84E-08 1.1E-08 1.63E-07 -5.42E-06
SQP SQP 2.32E+03 5.88E+00 0 0 0 0 1.73E+01 2.87E+00 2.28E+01 -4.38E+02
PM = Potential incidence of disease due to PM emissions; IR = Potential Human exposure efficiency relative to U235; ETP-fw = Potential comparative
Toxic Unit for ecosystems; HTP-c = Potential comparative Toxic Unit for humans (cancerogenic); HTP-nc = Potential comparative Toxic Unit for humans
(not cancerogenic); SQP = Potential soil quality index
Disclaimer 1 – for the indicator 'Potential Human exposure efficiency relative to U235'.This impact category deals mainly with the
eventual impact of low dose ionizing radiation on human health of the nuclear fuel cycle. It does not consider effects due to possible
nuclear accidents, occupational exposure or radioactive waste disposal in underground facilities. Potential ionizing radiation from the
soil, radon and from some construction materials is also not measured by this indicator.
Disclaimer 2 – for the indicators 'abiotic depletion potential for non-fossil resources', 'abiotic depletion potential for fossil resources',
'water (user) deprivation potential, deprivation-weighted water consumption', 'potential comparative toxic unit for ecosystems', 'potential
comparative toxic unit for humans – cancerogenic', 'Potential comparative toxic unit for humans - not cancerogenic', 'potential soil
quality index'. The results of this environmental impact indicator shall be used with care as the uncertainties on these results are high
as there is limited experience with the indicator.
6. LCA: Interpretation
Figure 1 illustrates the relative contributions of the different
modules along the life cycle of the declared products.
Figure 1: Relative environmental impacts of the different product life cycle (modules A1-C4). [1] The use of renewable
life cycle stages for the fixed flat roof window CFU primary energy is mainly caused by the share of renewable
energy in the electricity mix, thus the production stage and is
The largest part of environmental impacts – between 90% and the main driver of this impact category; also for the use of non-
rather100 % - is caused during production (modules A1-A3) of renewable primary energy, the production phase is the most
the flat roof window. No operational energy is used as the flat impacting life cycle stage.
roof window cannot be opened. Material use of primary energy is negligible and related to
Benefits and burdens beyond the system boundary (module D) plastic parts of the product and packaging material. The
are in the order of 0 % to about 130 % of the impacts over the material use of primary energy is transferred to its energy use
8 Environmental Product Declaration - VELUX A/S - VELUX flat roof window CFU
when the materials containing primary energy are incinerated
with energy recovery. [1] Benefits resulting from the recycling of plastics as well as
Non-hazardous waste as the quantitatively most relevant waste from the recycling of the electronic parts are disregarded due to
flows is mainly caused during the production of the glass and the lack of data on the recycling processes and related to the
during disposal of the product; hazardous and radio-active detailed composition of the electronic parts.
wastes are mainly caused by the European electricity mix.
7. Requisite evidence
to AltholzVO
7.1 Formaldehyde Not applicable; not tested based on applicable product
Not tested based on applicable product standard. standard. 7.4. Fire gas toxicity
Not tested based on applicable product standard. 7.5 VOC
7.2 MDI emissions
Not tested based on applicable product standard. 7.3 Not tested based on applicable product standard.
Checking of pre-treatment of substances used according
8. References
Product category rules of IBU methods.
IBU (2021) EAD 220062-00-0401
IBU (2021): General Instructions for the EPD Programme of the EAD 220062-00-0401, June 2017, rooflight with bonded or
Institut Bauen & Umwelt e.V. (General Instructions for the IBU mechanically fastened cover glass
EPD Programme). Version 2.0, Institut Bauen & Umwelt, Berlin
EN 16485
IBU (2017) DIN EN 16485:2014-07, Round and sawn timber -
IBU (2017): PCR Teil A: PCR Part A: Calculation rules for the Environmental Product Declarations - Product category rules
life cycle assessment and requirements for the project report. for wood and wood-based products for use in construction;
Version 1.8., Institut Bauen & Umwelt, Berlin. German version EN 16485:2014.
IBU (2021) ECHA-List
IBU (2021):PCR Part B: Requirements on the EPD for windows The Candidate List of substances of very high concern,
and doors. Version 2021/01, Institut Bauen & Umwelt, Berlin. available via https://echa.europa.eu/nl/-/four-newsubstances-
added-to-the-candidate-list.
Standards and legal documents
Regulation on biocidal products
EN 15804 REGULATION (EU) No 528/2012 OF THE EUROPEAN
DIN EN 15804+A2:2019, Sustainability of construction works - PARLIAMENT AND OF THE COUNCIL of 22 May 2012
Environmental product declarations - Core rules for the product concerning the making available on the market and use of
category construction products. biocidal products.
ISO 14025 Regulation (EU) Nr. 305/2011(CPR)
DIN EN ISO 14025:2006-07, Environmental labels and REGULATION (EU) No 305/2011 OF THE EUROPEAN
declarations - Type III Environmental declarations - Principles PARLIAMENT AND OF THE COUNCIL of 9 March 2011 laying
and procedures. down harmonised conditions for the marketing of construction
products and repealing Council Directive 89/106/EEC.
ISO 14044
DIN EN ISO 14044:2006-07, Environmental management - Life COUNCIL REGULATION (EU) No 333/2011
cycle assessment - Requirements and guidance (ISO COUNCIL REGULATION (EU) No 333/2011 of 31 March 2011
14044:2006); German and English versions EN ISO establishing criteria determining when certain types of scrap
14044:2006. metal cease to be waste under Directive 2008/98/EC of the
European Parliament and of the Council.
ISO 9001
DIN EN ISO 9001:2015, Quality management systems - European Waste List (Waste index)
Requirements. http://www.gesetze-im-internet.de/avv/anlage.htm
ISO 14001 Additional references
DIN EN ISO 14001:2015: Environmental management
systems - Requirements with guidance for use. Weidema et al. (2013)
Weidema, B., C. Bauer, R. Hischier, C. Mutel, T. Nemecek, J.
ISO 45001 Reinhard, C.O. Vadenbo, G. Wernet (2013): Overview and
ISO 45001:2018-03, Occupational health and safety methodology, Data quality guideline for the ecoinvent database
management systems - Requirements with guidance for use. version 3. ecoinvent report no. 1 (v3), St. Gallen, Schweiz.
EN 1873 ecoinvent 3.8
DIN EN 1873:2005, Prefabricated accessories for roofing - ecoinvent 3.8, LCA database, 12/2021. Ecoinvent centre,
Individual rooflights of plastics - Product specification and test Zürich.
9 Environmental Product Declaration - VELUX A/S - VELUX flat roof window CFU
Publisher
Institut Bauen und Umwelt e.V. +49 (0)30 3087748- 0
Hegelplatz 1 info@ibu-epd.com
10117 Berlin www.ibu-epd.com
Germany
Programme holder
Institut Bauen und Umwelt e.V. +49 (0)30 3087748- 0
Hegelplatz 1 info@ibu-epd.com
10117 Berlin www.ibu-epd.com
Germany
Author of the Life Cycle Assessment
Dr. Frank Werner - Umwelt & Entwicklung + 41 (0)44 241 39 06
Kammelenbergstrasse 30 frank@frankwerner.ch
9011 St. Gallen http://www.frankwerner.ch/
Switzerland
Owner of the Declaration
VELUX Group +4545164726
Ådalsvej 99 jakob.roerbech@velux.com
2970 Hørsholm www.velux.com
Denmark
10 Environmental Product Declaration - VELUX A/S - VELUX flat roof window CFU
