ENVIRONMENTAL PRODUCT DECLARATION
as per ISO 14025 and EN 15804+A2
Owner of the Declaration dormakaba International Holding GmbH
Publisher Institut Bauen und Umwelt e.V. (IBU)
Programme holder Institut Bauen und Umwelt e.V. (IBU)
Declaration number EPD-DOR-20210193-CBA2-EN
Issue date 07.10.2021
Valid to 06.10.2026
Access manager 92 00
dormakaba
www.ibu-epd.com | https://epd-online.com
General Information
dormakaba Access manager 92 00
Programme holder Owner of the declaration
IBU – Institut Bauen und Umwelt e.V. dormakaba International Holding GmbH
Hegelplatz 1 DORMA Platz 1
10117 Berlin 58256 Ennepetal
Germany Germany
Declaration number Declared product / declared unit
EPD-DOR-20210193-CBA2-EN 1 piece of the product: Access manager 92 00
This declaration is based on the product category rules: Scope:
Electronic and physical Access Control Systems, 01.08.2021 This EPD refers to a specific product manufactured by dormakaba. The
(PCR checked and approved by the SVR) production site is located in Villingen-Schwenningen (Germany).
The data represents the year 2020.
Issue date The owner of the declaration shall be liable for the underlying information
and evidence; the IBU shall not be liable with respect to manufacturer
07.10.2021
information, life cycle assessment data and evidences.
The EPD was created according to the specifications of EN 15804+A2. In
Valid to
the following, the standard will be simplified as EN 15804.
06.10.2026
Verification
The standard EN 15804 serves as the core PCR
Independent verification of the declaration and data according to ISO
14025:2011
internally X externally
Dipl.-Ing. Hans Peters
(Chairman of Institut Bauen und Umwelt e.V.)
Florian Pronold Dr.-Ing. Wolfram Trinius,
(Managing Director Institut Bauen und Umwelt e.V.) (Independent verifier)
1 Environmental Product Declaration - dormakaba - Access manager 92 00
Product
Product description/Product definition Peripherals Interface
The dormakaba access manager 92 00 fulfils all the • 1x RS-485
requirements of modern security systems. With its intelligent • 2x RS-232
decision logic and ability to be freely parametrised, it can • 2x coaxial for registration units (LEGIC / MIFARE)
control simple types of access points as well as more complex • 3x potential-free relays, 30 V AC/DC; max. 2 A
entrances to highly sensitive areas. Based on the latest • 4x digital inputs, 5V power supply integrated
operating system and transport layer security (TLS) encryption • 1x bus for extension modules
between the controller and host system, the IT security is state- • 1x tamper contact
of-the-art. With integrated mobile access, the access system
allows access via smartphone. The control electronics integrate Power supply
everything that is required to enable a connection to cloud • 10-34V DC
services via IoT. With its flexible and extendable design, it offers
a wide range of installation options. It can be installed locally as Installation
an individual device near an access point, in switch cabinets or Top hat rails as per EN 60715: TH35/(7.5/15)
centrally with extended input/output modules. Up to two Class of protection as per EN 60529: IP20
registration units can be connected directly and further access
readers via the RS-485 sub-bus. For the placing on the market The product is not harmonised in accordance with the
in the European Union/European Free Trade Association Construction Product Regulations (CPR) but in accordance with
(EU/EFTA) (with the exception of Switzerland) the following other provisions for harmonisation of the EU. Compliance with
legal provisions apply: the European Union Directive and technical specifications:
• Restriction of Hazardous Substances (RoHS) • EN 300330 V2.1.1
• Radio Equipment Directive (RED) • EN 301489-1 V2.2.0
The CE-marking takes into account the proof of conformity with • EN 301489-3 V2.1.1
the respective harmonized standards based on the legal • EN 50364:2010
provisions above. For the application and use the respective • EN 62368-1:2014
national provisions apply. The product is subject to CE marking according to the relevant
harmonization legislation.
Application
In addition, the product also conforms to the following
Flexible access control standards:
An access manager is installed in a protected environment and
• UL 294:2013
uses local or online decision logic to check whether an access
• UL 62368-1:2014
request via connected card readers is granted or rejected.
• CAN/CSA-22.2 No. 62368-1:2014
• FCC ID NVI-DKAM9200-K7
Door management
• Personnel interlock control
Base materials/Ancillary materials
• Door activation
The major material compositions of the product are listed
• Monitoring of door opening
below:
• Monitoring of door opening time
• Access monitoring Name Value Unit
Electronics 45 %
Alarm Management Paper 29 %
The access manager reports irregularities in access control or
Plastics 26 %
door management to the host computer. Tampering and
Steel <0,5 %
burglary attempts are reliably identified.
The product includes partial articles which contain substances
Technical Data listed in the Candidate List of REACH Regulation
The access manager 92 00 has the following technical 1907/2006/EC (date: 08.07.2021) exceeding 0.1 percentage by
properties: mass in the alloy: yes
Name Value Unit
• Lead titanium trioxide (O3PbTi): 12060-00-03
Operating Temperature 0 - 50 °C The Candidate List can be found on the ECHA website
Operating Humidity 5 - 85 % address: https:echa.europa.eu/de/home.
Width Dimension 125 mm
Reference service life
Height Dimension 99 mm
The reference service life of the dormakaba access manager
Depth Dimension 45 mm 92 00 is estimated to be 15 years. This number is based on the
Weight (without packaging) 0,18 kg support and service life and is not an estimated lifetime.
Weight (with packaging) 0,25 kg
Power consumption "idle mode" 5 W
Power consumption "on mode" 12 W
Host Interface
• Ethernet 10/100 Mbit/s
LCA: Calculation rules
2 Environmental Product Declaration - dormakaba - Access manager 92 00
Declared Unit Use stage - Module B6
The declared unit is 1 piece of the product: Access manager 92 The use stage related to the operation of the building includes:
00. — B6, operational energy use
Declared unit
End-of-life stage– Modules C1-C4 and D
Name Value Unit
The end-of-life stage includes:
Declared unit 1 pce.
— C1, de-construction, demolition:
Conversion factor to 1 kg (kg per declared unit) 4 - — C2, transport to waste processing;
Product weight including packaging 0,25 kg — C3, waste processing for reuse, recovery and/or recycling;
— C4, disposal;
System boundary
including provision and all transport, provision of all materials,
The type of EPD is: cradle to gate with options, modules C1–
products and related energy and water use.
C4, and module D (A1–A3 + C + D and additional modules: A4
+ A5 + B6)
Module D (Benefits and loads beyond the system boundary)
includes:
Production - Module A1-A3
— D, recycling potentials, expressed as net impacts and
The product stage includes:
benefits.
— A1, raw material extraction, processing and mechanical
treatments, processing of secondary material input (e.g.
Geographic Representativeness
recycling processes), — A2, transport to the manufacturer,
Land or region, in which the declared product system is
— A3, manufacturing and assembly including provision of all
manufactured, used or handled at the end of the product´s
materials, products and energy, as well as waste processing up
lifespan: Germany
to the end-of waste state.
Construction stage - Modules A4-A5 Comparability
The construction process stage includes:
Basically, a comparison or an evaluation of EPD data is only
— A4, transport to the building site; — A5, installation into the
possible if all the data sets to be compared were created
building; including provision of all materials, products and
according to EN 15804 and the building context, respectively
energy, as well as waste processing up to the end-of-waste
the product-specific characteristics of performance, are taken
state or disposal of final residues during the construction
into account. Background database: GaBi, SP40.
process stage.
LCA: Scenarios and additional technical information
Operational energy use (B6) and Operational water use
Characteristic product properties of biogenic carbon
(B7)
Information on describing the biogenic Carbon Content at The use stage is declared for 15 years.
factory gate
Name Value Unit
Name ValueUnit
Energy consumption for 1 year 54.02 kWh
kg
Biogenic carbon content in product - on mode per day 4 h
C
idle mode 20 h
Biogenic carbon content in accompanying kg
0.03 on mode power 12 W
packaging C
idle mode 5 W
Note: 1 kg of biogenic carbon is equivalent to 44/12 kg of CO .
2 Days per year in use 365 days
End of life (C1-C4)
The following technical scenario information is required for the
C1: The product dismantling from the building is done manually
declared modules.
without environmental burden.
Transport to the building site (A4)
Name Value Unit
Name Value Unit Energy recovery (Plastic) 0.06 kg
Litres of fuel per 1 kg (truck) 0.00276 l/100km Recycling (Steel) 0,01 kg
Transport distance (truck) 750 km Recycling and landfilling (Electronics) 0,11 kg
Capacity utilisation (including empty runs) 51 % Transportation to Waste Processing Site 50 km
Transort distance (ship) 1000 km
Region for end of life: Global
Installation into the building (A5)
Reuse, recovery and/or recycling potentials (D), relevant
Name Value Unit
scenario information
Waste Packaging (paper) 0.0716 kg Collection rate is 100%.
Reference service life
Name Value Unit
Life Span according to the manufacturer 15 a
3 Environmental Product Declaration - dormakaba - Access manager 92 00
LCA: Results
DESCRIPTION OF THE SYSTEM BOUNDARY (X = INCLUDED IN LCA; MND = MODULE OR INDICATOR NOT DECLARED; MNR
= MODULE NOT RELEVANT)
Benefits and
Construction loads beyond
Product stage Use stage End of life stage
process stage the system
boundaries
la ire ta m w a Ry lp p u s tro p s n a rT g n iru tc a fu n a M e h t m o rf tro p s n a rTe tis e h t o t e ta g y lb m e s s A e s U e c n a n e tn ia M ria p e R tn e m e c a lp e R tn e m h s ib ru fe R y g re n e la n o ita re p Oe s u re ta w la n o ita re p Oe s u n o itc u rts n o c -e Dn o itilo m e d tro p s n a rT g n is s e c o rp e ts a W la s o p s iD -e s u e R-y re v o c e R-g n ilc y c e Rla itn e to p
A1 A2 A3 A4 A5 B1 B2 B3 B4 B5 B6 B7 C1 C2 C3 C4 D
X X X X X MND MND MNR MNR MNR X MND MND X X X X
RESULTS OF THE LCA - ENVIRONMENTAL IMPACT according to EN 15804+A2: 1 piece Access manager 92 00
Parameter Unit A1-A3 A4 A5 B6 C2 C3 C4 D
GWP-total kg CO 2 eq 5.92E+00 1.72E-02 1.02E-01 4.13E+02 7.82E-04 2.2E-01 6.87E-05 -3.59E-01
GWP-fossil kg CO 2 eq 5.93E+00 1.65E-02 2.54E-03 4.11E+02 7.47E-04 2.2E-01 6.83E-05 -3.59E-01
GWP-biogenic kg CO 2 eq -1.66E-02 7.26E-04 9.9E-02 8.16E-01 3.45E-05 5.13E-06 2.33E-07 3.05E-04
GWP-luluc kg CO 2 eq 8.99E-03 3.9E-07 1.67E-06 5.78E-01 1.78E-08 1.25E-05 1.96E-07 -4.83E-04
ODP kg CFC11 eq 7.77E-10 1.73E-18 1.83E-17 6.2E-12 7.89E-20 1.11E-16 2.53E-19 -2.1E-15
AP mol H+ eq 3.33E-02 4.58E-05 2.84E-05 1.83E+00 7.48E-07 3.92E-05 4.9E-07 -4.34E-03
EP-freshwater kg P eq 4.3E-05 3.54E-09 3.58E-09 7.83E-04 1.6E-10 1.77E-08 1.17E-10 -3.21E-07
EP-marine kg N eq 5.84E-03 1.29E-05 1.03E-05 3E-01 2.38E-07 8.85E-06 1.26E-07 -3.39E-04
EP-terrestrial mol N eq 6.22E-02 1.43E-04 1.28E-04 3.23E+00 2.64E-06 1.79E-04 1.38E-06 -3.65E-03
kg NMVOC
POCP 1.71E-02 3.63E-05 2.72E-05 8.67E-01 6.73E-07 2.45E-05 3.82E-07 -1.13E-03
eq
ADPE kg Sb eq 1.14E-02 2.32E-01 3.2E-02 6.19E+03 1.06E-02 1.02E-01 8.96E-04 -4.93E+00
ADPF MJ 7.27E+01 4.91E-10 2.89E-10 8.48E-05 2.24E-11 1.52E-09 6.13E-12 -1.95E-04
m3 world eq
WDP 1.42E+00 3.22E-05 1.26E-02 8.74E+01 1.46E-06 2.25E-02 7.16E-06 -1.26E-01
deprived
GWP = Global warming potential; ODP = Depletion potential of the stratospheric ozone layer; AP = Acidification potential of land and water; EP =
Eutrophication potential; POCP = Formation potential of tropospheric ozone photochemical oxidants; ADPE = Abiotic depletion potential for non-fossil
resources; ADPF = Abiotic depletion potential for fossil resources; WDP = Water (user) deprivation potential)
RESULTS OF THE LCA - INDICATORS TO DESCRIBE RESOURCE USE according to EN 15804+A2: 1 piece Access manager 92
00
Parameter Unit A1-A3 A4 A5 B6 C2 C3 C4 D
PERE MJ 1.73E+01 7.33E-04 8.65E-01 2.32E+03 3.34E-05 4.46E-02 1.17E-04 -7.8E-01
PERM MJ 8.77E-01 0 -8.59E-01 0 0 -1.8E-02 0 0
PERT MJ 1.82E+01 7.33E-04 5.82E-03 2.32E+03 3.34E-05 2.66E-02 1.17E-04 -7.8E-01
PENRE MJ 6.9E+01 2.32E-01 3.21E-02 6.2E+03 1.06E-02 3.86E+00 8.96E-04 -4.93E+00
PENRM MJ 3.76E+00 0 0 0 0 -3.76E+00 0 0
PENRT MJ 7.27E+01 2.32E-01 3.21E-02 6.2E+03 1.06E-02 1.02E-01 8.96E-04 -4.93E+00
SM kg 0 0 0 0 0 0 0 0
RSF MJ 0 0 0 0 0 0 0 0
NRSF MJ 0 0 0 0 0 0 0 0
FW m3 3.66E-02 1.32E-06 2.96E-04 3.16E+00 5.99E-08 5.39E-04 2.26E-07 -2.49E-03
PERE = Use of renewable primary energy excluding renewable primary energy resources used as raw materials; PERM = Use of renewable primary
energy resources used as raw materials; PERT = Total use of renewable primary energy resources; PENRE = Use of non-renewable primary energy
excluding non-renewable primary energy resources used as raw materials; PENRM = Use of non-renewable primary energy resources used as raw
materials; PENRT = Total use of non-renewable primary energy resources; SM = Use of secondary material; RSF = Use of renewable secondary fuels;
NRSF = Use of non-renewable secondary fuels; FW = Use of net fresh water
RESULTS OF THE LCA – WASTE CATEGORIES AND OUTPUT FLOWS according to EN 15804+A2:
1 piece Access manager 92 00
Parameter Unit A1-A3 A4 A5 B6 C2 C3 C4 D
HWD kg 6.15E-06 2.26E-11 4.72E-11 2.87E-06 1.03E-12 3.89E-10 1.37E-11 -1.32E-08
NHWD kg 2.07E-01 2.38E-05 3.18E-03 3.87E+00 1.08E-06 2.29E-02 4.5E-03 -5.39E-02
RWD kg 1.67E-03 2.5E-07 1.68E-06 7.18E-01 1.14E-08 3.79E-06 1.02E-08 -1.67E-04
CRU kg 0 0 0 0 0 0 0 0
MFR kg 0 0 0 0 0 8.76E-02 0 0
MER kg 0 0 0 0 0 0 0 0
EEE MJ 1.07E-01 0 1.54E-01 0 0 0 0 0
EET MJ 1.95E-01 0 2.79E-01 0 0 0 0 0
4 Environmental Product Declaration - dormakaba - Access manager 92 00
HWD = Hazardous waste disposed; NHWD = Non-hazardous waste disposed; RWD = Radioactive waste disposed; CRU = Components for re-use;
MFR = Materials for recycling; MER = Materials for energy recovery; EEE = Exported electrical energy; EET = Exported thermal energy
RESULTS OF THE LCA – additional impact categories according to EN 15804+A2-optional:
1 piece Access manager 92 00
Parameter Unit A1-A3 A4 A5 B6 C2 C3 C4 D
Disease
PM 3.35E-07 5.97E-10 1.57E-10 2.56E-05 3.93E-12 5.01E-10 6.06E-12 -3.51E-08
incidence
IR kBq U235 eq 1.61E-01 3.57E-05 2.61E-04 1.16E+02 1.63E-06 3.42E-04 1.05E-06 -2.61E-02
ETP-fw CTUe 3.91E+01 1.65E-01 1.52E-02 2.28E+03 7.51E-03 3.83E-02 5.12E-04 -2.27E+00
HTP-c CTUh 1.94E-09 3.1E-12 8.04E-13 8.34E-08 1.41E-13 3.32E-12 7.58E-14 -1.53E-10
HTP-nc CTUh 1.09E-07 1.33E-10 3.49E-11 3.32E-06 6.04E-12 3.36E-10 8.36E-12 -1.22E-08
SQP SQP 2.4E+01 5.98E-04 8.5E-03 1.71E+03 2.72E-05 3.06E-02 1.87E-04 -2.1E+00
PM = Potential incidence of disease due to PM emissions; IR = Potential Human exposure efficiency relative to U235; ETP-fw = Potential comparative
Toxic Unit for ecosystems; HTP-c = Potential comparative Toxic Unit for humans (cancerogenic); HTP-nc = Potential comparative Toxic Unit for humans
(not cancerogenic); SQP = Potential soil quality index
Disclaimer 1 – for the indicator IRP
This impact category deals mainly with the eventual impact of low dose ionizing radiation on human health of the nuclear fuel cycle. It
does not consider effects due to possible nuclear accidents, occupational exposure nor due to radioactive waste disposal in
underground facilities. Potential ionizing radiation from the soil, from radon and from some construction materials is also not measured
by this indicator.
Disclaimer 2 – for the indicators ADPE, ADPF, WDP, ETP-fw, HTP-c, HTP-nc, SQP
The results of this environmental impact indicator shall be used with care as the uncertainties on these results are high or as there is
limited experience with the indicator. This EPD was created using a software tool.
References
Standards (IP 20).
CAN/CSA-22.2 No. 62368-1 EN 60715
CAN/CSA-22.2 No. 62368-1:2014, Audio/video, information and EN 60715:2018, Dimensions of low-voltage switchgear and
communication technologyequipment — Part 1: Safety controlgear - Standardized mounting on rails for mechanical
requirements. support of switchgear, controlgear and accessories
EN 15804:2019+A2 EN 62368-1
EN 15804:2019+A2 (in press), Sustainability of construction EN 62368-1:2014, Audio/video, information and communication
works — Environmental Product Declarations — Core rules for technology equipment - Part 1: Safety requirements.
the product category of construction products.
ISO 14025
EN 301489-1 V2.2.0 DIN EN ISO 14025:2011-10, Environmental labels and
ElectroMagnetic Compatibility (EMC) standard for radio declarations — Type III environmental declarations —
equipment and services - Part 1: Common technical Principles and procedures.
requirements - Harmonised Standard covering the essential
requirements of article 3.1(b) of Directive 2014/53/EU and the Radio Equipment Directive (RED)
essential requirements of article 6 of Directive 2014/30/EU. Directive 2014/53/EU of the European Parliament and of the
Council of 16 April 2014 on the harmonisation of the laws of the
EN 301489-3 V2.1.1 Member States relating to the making available on the market
ElectroMagnetic Compatibility (EMC) standard for radio of radio equipment and repealing Directive 1999/5/EC.
equipment and services - Part 3: Specific conditions for Short-
Range Devices (SRD) operating on frequencies between 9 kHz Registration, Evaluation, Authorisation and Restriction of
and 246 GHz - Harmonised standard covering the essential Chemicals (REACH)
requirements of article 3.1(b) of Directive 2014/53/EU. Regulation (EC) No 1907/2006 of the European Parliament and
of the Council on the Registration, Evaluation, Authorisation
EN 300330 V2.1.1 and Restriction of Chemicals (REACH).
Short Range Devices (SRD) - Radio equipment in the
frequency range 9 kHz to 25 MHz and inductive loop systems in Restriction of Hazardous Substances (RoHS)
the frequency range 9 kHz to 30 MHz - Harmonised Standard Directive on the restriction of the use of certain hazardous
covering the essential requirements of article 3.2 of the substances in electrical and electronic equipment (RoHS),
Directive 2014/53/EU. Directive (EU) No 2011/65.
EN 50364 UL 294
EN 50364:2010, Limitation of human exposure to UL 294:2013, Standard for Safety Access Control System Unit.
electromagnetic fields from devices operating in the frequency
range 0 Hz to 300 GHz, used in Electronic Article Surveillance UL 62368-1
(EAS), Radio Frequency Identification (RFID) and similar UL 62368:2014, Standard for Audio/video, information and
applications. communication technology equipment - Part 1: Safety
requirements.
EN 60529
EN 60529:2014, Degrees of protection provided by enclosures Further References
5 Environmental Product Declaration - dormakaba - Access manager 92 00
LCA-tool dormakaba
IBU 2016 LCA tool, version 1.0.
Institut Bauen und Umwelt e.V.: General Instructions for the Developed by Sphera Solutions GmbH.
EPD programme of Institut Bauen und Umwelt e.V. Version
2.0., Berlin: Institut Bauen und Umwelt e.V., 2021. www.ibu- PCR Part A
epd.com PCR – Part A:
GaBi ts software Calculation Rules for the Life Cycle As-sessment and
Sphera Solutions GmbH Requirements on the Project Re-port according to EN
Gabi Software System and Database for Life Cycle Engineering 15804+A2:2019, Version 1.0, Institut Bauen und Umwelt e.V.,
1992-2020 Version 10.0.0.71 University of Stuttgart Leinfelden- www.ibu-epd.com.
Echterdingen
PCR Part B
GaBi ts documentation
GaBi life cycle inventory data documentation (https://www.gabi- PCR – Part B: Requirements on the EPD for Building Hardware
software.com/support/gabi/gabi-database-2020-lci- product, version 1.3, Institut Bauen und Umwelt e.V., www.ibu-
documentation/). epd.com, 2019.
6 Environmental Product Declaration - dormakaba - Access manager 92 00
Publisher
Institut Bauen und Umwelt e.V. +49 (0)30 3087748- 0
Hegelplatz 1 info@ibu-epd.com
10117 Berlin www.ibu-epd.com
Germany
Programme holder
Institut Bauen und Umwelt e.V. +49 (0)30 3087748- 0
Hegelplatz 1 info@ibu-epd.com
10117 Berlin www.ibu-epd.com
Germany
Author of the Life Cycle Assessment
Sphera Solutions GmbH +49 711 341817-0
Hauptstraße 111- 113 info@sphera.com
70771 Leinfelden-Echterdingen www.sphera.com
Germany
Owner of the Declaration
dormakaba International Holding GmbH +49 2333 793-0
DORMA Platz 1 info.de@dormakaba.com
58256 Ennepetal www.dormakaba.com
Germany
7 Environmental Product Declaration - dormakaba - Access manager 92 00
