ENVIRONMENTAL PRODUCT DECLARATION
as per ISO 14025 and EN 15804+A2
Owner of the Declaration Unilin B.V. Division Panels
Publisher Institut Bauen und Umwelt e.V. (IBU)
Programme holder Institut Bauen und Umwelt e.V. (IBU)
Declaration number EPD-UNI-20230376-IBJ2-EN
Issue date 31.10.2023
Valid to 30.10.2028
Unilin Chipboard
Unilin B.V. Division Panels
www.ibu-epd.com | https://epd-online.com
1. General Information
Unilin B.V. Division Panels Unilin Chipboard
Programme holder Owner of the declaration
IBU – Institut Bauen und Umwelt e.V. Unilin B.V. Division Panels
Hegelplatz 1 Ooigemstraat 3
10117 Berlin 8710 Wielsbeke
Germany Belgium
Declaration number Declared product / declared unit
EPD-UNI-20230376-IBJ2-EN 1 m³ Unilin chipboard (676 kg/m³)
This declaration is based on the product category rules: Scope:
Wood-based panels, 01.08.2021 The scope of this EPD extends to all Unilin raw chipboards. The declared
(PCR checked and approved by the SVR) values refer to the sales-weighted average product. These chipboards are
produced in following manufacturing sites:
• SPANO, Oostrozebeke, Belgium
Issue date
• BOSPAN, Wielsbeke, Belgium
31.10.2023
The owner of the declaration shall be liable for the underlying information
and evidence; the IBU shall not be liable with respect to manufacturer
Valid to information, life cycle assessment data and evidences.
30.10.2028
The EPD was created according to the specifications of EN 15804+A2. In
the following, the standard will be simplified as EN 15804.
Verification
The standard EN 15804 serves as the core PCR
Independent verification of the declaration and data according to ISO
14025:2011
internally X externally
Dipl.-Ing. Hans Peters
(Chairman of Institut Bauen und Umwelt e.V.)
Florian Pronold Mr Olivier Muller,
(Managing Director Institut Bauen und Umwelt e.V.) (Independent verifier)
1 Environmental Product Declaration - Unilin B.V. Division Panels - Unilin Chipboard
2. Product
• P6 (and U7-U8-U9): heavy-duty load-bearing boards for
2.1 Product description/Product definition use in dry conditions.
Unilin Chipboards are wood-based panels with 3 layers: two
surface layers with a fine structure and a core layer with a The surface variety accommodates the use of a versatile range
coarser structure. The layers consist of wood chips that are of finishes and coatings, making the material easy to use in
bonded by a thermo-harding glue and mixed with additives to many different designs and applications.
add application-specific properties such as fire retardancy or
moisture resistance. 2.3 Technical Data
Technical characteristics vary by product variant and thickness.
More detailed product-specific data, technical data sheets and
For the placing on the market of the product in the European the CE declaration of performance are available on
Union/European Free Trade Association (EU/EFTA) (with the www.unilinpanels.com.
exception of Switzerland) Regulation (EU) No. 305/2011 (CPR)
Constructional data
applies. The product needs a declaration of performance
The table below summarizes the technical performance of
according:
Unilin's raw chipboard range for some parameters. The values
• EN 13986:2004+A1:2015, Wood-based panels for use below apply to the product range. More detailed information on
in construction – Characteristics, valuation of conformity these ranges and additional parameters (e.g. swelling,
and marking biological durability, etc.) is available at the product's
• EN 16368:2014, Lightweight Particleboards – "Declaration Of Performace" on www.unilinpanels.com. Specific
Specifications properties of the declared sales-weighted product are available
• EN 312:2010-12, Particleboards – Specifications in 3.10.
Name Value Unit
For the application and use the respective national provisions
Gross Density (EN 323) 430 - 760 kg/m³
apply.
Bending strength (EN 310) 2 - 20 N/mm²
The results in this EPD refer to the environmental impact of a E-modulus (EN 310) 375 - 3500 N/mm²
raw chipboard with a sales-weighted average. The composition Material dampness at
6 - 10 %
of this product was obtained by averaging Unilin's entire delivery (EN 322)
chipboard portfolio using the annual sales volumes as weighing
Tensile strength (EN 319) 0.14 - 0.7 N/mm²
factor. The declared impact is thus representative for the
Thermal conductivity (EN
following commercial references: 0.12 - 0.14 W/(mK)
13986)
• Air Ultralight/Extemelight
Water vapour diffusion
• Air/Air Light
resistance factor (EN 12 - 50
• Liso (LF/LF+)
13986)
• Belspan (LF/LF3/LF+) (TG)
Sound absorption 250 -
• Qualirack (LF/LF+) (TG) 0.10
500 HZ (EN 13986)
• SB4 (TG)
• Systemfloor (LF/LF+) Sound absorption 1000 - 0.25
• Systemfloor Plus (LF/LF+) (Basic) 2000 HZ (EN 13986)
• Systemfloor HD (LF/LF+) (TG) E1(*); E0.5 (**);
• Hydrolis (UC) (LF3/LF4/LF/LF+) (TG) Formaldehyde CARB/TSCA Title VI
• Durelis (UC) (LF/LF+) (TG) (***);F****(****)
• Antivlam (LF/LF+) (TG)
Different formaldehyde emission standards are available :
• Hydroflam (TG)
(*) E1 - According to EN 13986+A1:2015 :
The values for specific commercial references can vary from • a limit value of 0.1 ppm may not be exceeded by EN
the declared ones. Please contact Unilin's sales team or 717-1 emission chamber method OR
info.panels@unilin.com for more information. • a limit value of 8 mg HCHO/100 g according to ISO
12460-5
2.2 Application (**) E0.5 - According to the ChemVerbotsV :
Unilin Chipboards are used in structural and non-structural • a limit value of 0.1 ppm according to EN 16516 OR
applications for example furniture, interior and building • a limit value of 0.05 ppm according to EN 717-1
applications : (***) CARB 2/TSCA Title VI - According to California Air
• LP1: General purpose lightweight boards for use in dry Resources Board & the US Toxic Substances Control Act
conditions. (TSCA Title VI) :
• LP2: general purpose (including furniture) lightweight • a limit value of 0.09 ppm according to ASTM E1333 or
boards for use in dry conditions. ASTM D6007
• P1: General purpose boards for use in dry conditions. (****) F**** - According to Japanese standard JIS A 5908
• P2: Boards for interior furnishings (including furniture)
• a limit value of 0.3 mg/L according to JIS A 1460
for use in dry conditions.
desiccator
• P3: Boards for non-loadbearing purposes for use in
Performance data are consistent with the product's declaration
humid conditions.
of performance with respect to its essential characteristics
• P4: Boards for load-bearing purposes for use in dry
according to:
conditions.
• P5: Load-bearing boards for use in humid conditions. • EN 13986:2004+A1:2015, Wood-based panels for use
in construction – Characteristics, valuation of conformity
2 Environmental Product Declaration - Unilin B.V. Division Panels - Unilin Chipboard
and marking 5. The endless board that leaves the press is cut into large
• EN 16368:2014, Lightweight Particleboards – panels and passively cooled.
Specifications 6. After cooling down, the panels can be sanded, cut to
• EN 312:2010, Particleboards – Specifications final size, and optionally finished further depending on
the intended application.
2.4 Delivery status
Unilin's chipboards are available in a diverse range of
dimensions:
• Length: 600 mm - 6700 mm
2.7 Environment and health during manufacturing
• Width: 600 mm - 2660 mm
Unilin's plant management policy is fully integrated in the daily
• Thickness: 8 - 54 mm
operation and governance of its production plants. The aim is to
adhere to legal requirements, minimize negative environmental
Please contact Unilin's sales team or info.panels@unilin.com
effects on its neighbors, co-workers and surroundings, and
for more information on available dimensions of specific
constantly improve environmental performance. The plants are
products.
ISO 9001 certified.
2.5 Base materials/Ancillary materials
The table below details the sales-weighted average The implementation of Unilin's One Home Sustainability
composition of the Unilin Chipboard. This chipboard has a Strategy and its Zero Harm Safety Policy have further set clear
density of 676 kg/m³ and consists of recycled and fresh wood, targets to among others reduce the carbon footprint of its
(melamine) urea formaldehyde glue ((M)UF), additives and production activities, improve the overall resource efficiency
moisture. The additives added depend heavily on the specific and enhance the safety and well-being at its production sites.
commercial reference (e.g. wax emulsion, fire retardant based
2.8 Product processing/Installation
on inorganic salts).
The Unilin Chipboard can be processed (e.g. sawing, milling,
Name Value Unit
drilling) using common utility tools and machinery. It is advised
Recycled Wood 78 % to wear a dust mask when tools are used without dust
Fresh wood 7 % extraction. More specific processing and health information is
(M)UF glue 8 % available at www.unilinpanels.com.
Additives 1 %
2.9 Packaging
Moisture 6 % Product packaging is used to protect the product from damage
The chipboard is primarily made up of recycled wood, during transport. Wood-based chipboards, cardboard,
accounting for 95 % of the total wood composition. 88 % stretchfoil and PET packaging straps are used as packaging
consists of post-consumer recycled wood, while the remaining materials.
7 % is coming from pre-consumer sources. These post-
2.10 Condition of use
consumer streams are composed of recycled wood, containing
The product's composition remains unchanged during its use
legacy fossil-based substances (e.g. glue and other additives),
and is therefore the same as stated in section 2.5. The glue and
along with other types of demolition waste. Unilin's state-of-the-
additives are permanently bonded to the wood through an
art recycling unit employs a variety of methods to eliminate
irreversible curing process.
these impurities, resulting in chipboards of exceptional quality
and safety.
2.11 Environment and health during use
Based on current knowledge, using the Unilin Chipboard as
The used fresh wood is 100 % recovered wood, predominantly
intended poses no risks to health, water, air or soil. Small
sourced from sustainable forest management activities and
amounts of natural wood constituents could potentially be
sawmills (residues & co-products), and mainly consists of
released, but aside from negligible amounts of formaldehyde,
spruce, oak and pine.
no harmful emissions have been detected.
The composition of specific commercial references can differ
2.12 Reference service life
from the values depicted above and can be obtained by
The reference service life (RSL) of the product depends
reaching out to info.panels@unilin.com.
significantly on its field of use. Please contact Unilin's sales
team or info.panels@unilin.com for more specific information
Unilin's chipboard range contains no Substances of Very High
on the product's lifespan in a given set of conditions.
Concern (SVHCs) or Category 1A or 1B CMR-substances (as
defined by ECHA) above 0.1 % by weight: No
The chipboard's RSL can vary from 10 to 50 years depending
The chipboards further contain no biocides as defined under
on its area of application; according to the BBSR table "BNB
the EU Biocidal Products Ordinance No. 528/2012 nor are the
Nutzungsdauern von Bauteilen (2017)".
boards treated with such substances.
2.13 Extraordinary effects
2.6 Manufacture
Fire
1. After roughly cutting, sorting and cleaning, the wood is The fire resistance of the Unilin Chipboard depends heavily on
cut into small chips. its chemical composition (i.e. presence of fire retardants). The
2. The chips are dried to the required moisture content. products have the following fire behaviour (according to
3. The dry chips are mixed with a thermohardening glue EN13501-1):
and additives.
4. The mixture is spread out in a 3 layer cake shaped CE AVCP Class 4 :
board and compressed at high pressure and
• Standard/Moisture Resistant chipboards (excl. fire
temperature to bind the wood particles and the glue into
retardant): D-s2,d0 (≥ 9mm/ Bulk density > 600 kg/m³)
a solid chipboard.
3 Environmental Product Declaration - Unilin B.V. Division Panels - Unilin Chipboard
selective dismantling/sorting takes place. After collection, the
CE AVCP Class 1 : end-of-life chipboard can be reused for the same (or different)
purpose if possible. The end-of-life material can also be
• Antivlam: B-s1,d0 (10 - 25 mm)
recycled into a new chipboard, replacing fresh wood chips.
• Hydroflam: B-s2,d0 (10 - 22 mm)
Energy Recovery
Fire reaction classes are part of the CE Declaration of
In line with the cascading use of wood-based products, the
Performance available on Unilin Panels website
reuse/recycling of end-of-life chipboard should be prioritized.
www.unilinpanels.com.
However, if this is not feasible, the chipboard can be used as a
secondary fuel in approved energy power plants. Its relatively
Water
high calorific value enables power plants to effectively produce
The Unilin Chipboard does not contain substances that may
renewable heat and electricity.
potentially contaminate water through leaching. However, it is
important, to ensure that the product is not subjected to
2.15 Disposal
continuous exposure to moisture. Prolonged contact with water
Jobsite and post-consumer chipboard waste (e.g. from
may result in the degradation of the product.
demolition projects) should be reused/recycled where possible,
in line with the cascade principle. Should this not be possible,
Mechanical destruction
the waste must be utilized for energy recovery as opposed to
When subjected to mechanical stress, the product displays a
being landfilled (in accordance with EWC waste codes
tendency towards brittleness. This could result in the formation
170201/030105).
of splinters and sharp broken edges, which may pose a risk of
Waste from packaging materials, which protect the product
injury. The product's ability to withstand mechanical impact is
from damage during transport, can be reused and recycled if
directly related to its respective board type, as indicated in
sorted correctly.
section 2.1.
2.16 Further information
2.14 Re-use phase
Please contact Unilin's sales team or reach out to
Reuse/recycling
info.panels@unilin.com for additional information.
When a building or furniture has reached its end-of-life phase,
the Unilin chipboard can easily be abstracted and collected if
3. LCA: Calculation rules
plants A&S and A&U generate renewable energy and heat from
3.1 Declared Unit these waste streams, which are directly supplied to Unilin's
The declared information and values in this Environmental chipboard plants. Any remaining energy needs are met through
Product Declaration refer to 1 m³ of Unilin Chipboard with a the local grid in Belgium.
sales-weighted average composition and density of 676 kg/m³.
Declared unit and mass reference C1: Deconstruction/Demolition stage
It is assumed that the end-of-life chipboard is manually
Name Value Unit
dismantled from the building/furniture. The efforts involved in
Declared unit 1 m3 this process are considered negligible, leading to the absence
Gross density 676 kg/m3 of a declared environmental impact arising from the dismantling
of the product.
Other declared units are allowed if the conversion is shown
transparently.
C2: Transport to Waste Processing
This life cycle stage describes the impact of the end-of-life
The composition of the Unilin Chipboard, for which values are
chipboard's transport from the demolition site to the waste
declared in this EPD, was obtained by averaging Unilin's entire
processing facility. A representative distance of 50 km is
chipboard portfolio based on the annual sales volumes. The
assumed.
product is produced at the SPANO and BOSPAN plants, which
are both in the scope of this declaration.
C3: Waste Processing
3.2 System boundary Processing of the post-consumer chipboard waste involves
(preliminary) sorting and shredding of the material. As an end-
This is a cradle-to-gate EPD with options, including the
of-life chipboard is either recycled or energetically recovered,
following life cycle phases A1 - A3, C1 - C4 and D. The
the material leaves the system as a secondary material or fuel
following processes have been considered for each of the
in module C3. The impact of both end-of-life scenarios is
modules:
declared in section 5. Material inherent properties (e.g. biogenic
carbon and primary energy content) are thus exported from the
A1 - A3: Product Stage
system in C3.
The production stage encompasses the extraction of raw
materials (i.e. wood, glue, additives), their transportation to the
C4: Waste Disposal
production plants, and the subsequent manufacturing of the
This module describes the loads and emissions attributed to
product. The required energy for production, ancillary materials,
the disposal of the product after waste processing. As the end-
and production emissions are included. Energy and material
of-life product leaves the system in C3 as secondary material or
input/output data were obtained from Unilin's chipboard
fuel, no environmental impact is declared in C4.
factories (SPANO and BOSPAN) as well as Unilin's glue
factory.
D: Loads and Benefits beyond the System Boundaries
Module D describes the loads and benefits related to the use of
A large share of the supplied production energy is derived from
the end-of-life chipboard either as a secondary material or as a
renewable sources. These consist of post-consumer woody
secondary fuel. The latter involves the energy recovery of post-
waste streams, which are not recyclable. The adjacent biomass
4 Environmental Product Declaration - Unilin B.V. Division Panels - Unilin Chipboard
consumer chipboard waste. Here it is assumed that the end-of- with ISO 14044. Primary data was directly gathered from the
life product replaces an European-averaged mix of electricity designated person at Unilin's chipboard and glue plants. It was
and heat. When used as a secondary material, the impact of ensured that the collected data accurately represented reality,
substituting fresh wood chips is considered. so it can be assumed that the used primary data is of high
quality.
The system boundary between subsequent systems is defined
in accordance with EN 15804+A2, i.e. when the material The technological, geographical, and time-related
reaches its end-of-waste state. During A1 - A3, the recycled representativeness of background data (e.g. from EcoInvent)
wood input is considered as end-of-waste after (preliminary) was verified, as stated in EN 15804+A2.
sorting and shredding in the previous system. Similarly, end-of-
life chipboard reaches its end-of-waste state after sorting and 3.7 Period under review
shredding the waste, as inventoried in C3. The end-of-life Primary data, needed to calculate the LCA of the system under
chipboard leaves the current system at module C3 and enters a study, was collected for the year 2020 from the BOSPAN,
subsequent system as a secondary material or fuel. SPANO and Unilin's glue production facility.
3.3 Estimates and assumptions 3.8 Geographic Representativeness
Specific, primary data have been used to the highest extent Land or region, in which the declared product system is
possible. In case of absence, estimates and assumptions were manufactured, used or handled at the end of the product´s
made to model reality as closely as possible. These lifespan: Belgium
assumptions are based on publicly available data and literature.
Generic dataset from the EcoInvent 3.8. database have been
3.9 Allocation
used to model the impact of some raw materials and process-
In line with the EN 15804+A2 and EN 16485, the biogenic
related parameters for which specific data was lacking.
carbon and primary energy content of the recycled and fresh
wood have been balanced over the product's entire life cycle
End-of-life chipboard can leave the product system in C3 as a
(A1 - C4) based on their inherent material characteristics and
secondary fuel, for which the benefits and loads are inventoried
underlying physical flows. Fresh wood inventories were taken
in module D. Here it is assumed that the secondary fuel
from EcoIvent 3.8. Here, it was made sure that the biogenic
substitutes electricity and heat in accordance with an average
carbon and energy content reflect the physical relationships of
mix available on the European grid.
the different wood-based materials.
3.4 Cut-off criteria
All in- and outputs to the system under study have been The output of Unilin's chipboard plants consists of two products,
included in the LCA. Primary data was used to the highest i.e. the chipboard and post-consumer metal-based products
extent possible. If primary data was lacking, secondary data (i.e. by-product). The latter is extracted from the post-consumer
from EcoInvent was resorted to. Conservative assumptions wood waste of which the Unilin Chipboard is largely composed.
were made using average or generic data in case of data gaps. These metal-based materials are abstracted from the woody
These assumptions are based on publicly available (literature waste streams in module A3. Since the difference in revenue
reported) data. As such, all processes, materials, or emissions between the 2 outputs is relatively significant, the allocation of
expected to have a significant contribution to the environmental the relevant production-related process and emissions was
impact of the system under study were considered in the LCA. carried out based on their respective economic values (as
The total sum of omitted flows can therefore be deemed as described in EN 15804).
significantly below the 5 % threshold of the system's energy
and mass input, as stated in the EN 15804+A2. The system boundary (and subsequent allocation) relating to
the flow of post-consumer wood and end-of-life product are as
3.5 Background data described in section 3.2.
The relevant background data was either taken from the
3.10 Comparability
EcoInvent 3.8. database or peer-reviewed literature sources.
Measures were taken to ensure that the used secondary data Basically, a comparison or an evaluation of EPD data is only
was no more than 10 years old. These data types allowed to possible if all the data sets to be compared were created
map the background system in the LCA of the product under according to EN 15804 and the building context, respectively
study. the product-specific characteristics of performance, are taken
into account. Background data was used from the EcoInvent
3.6 Data quality 3.8. database.
Data collection and necessary calculations were done in line
4. LCA: Scenarios and additional technical information
Note: 1 kg biogenic carbon is equivalent to 44/12 kg CO .
2
Characteristic product properties of biogenic carbon
The values declared below describe the amount of biogenic
carbon and stored biogenic CO in the building product under
2 The following technical information is a basis for the declared
study when it leaves the factory gate. The values relate to 1 m³ modules or can be used for developing specific scenarios in the
of Unilin chipboard, with a sales-weighted average composition. context of a building assessment if modules are not declared
Biogenic carbon content at factory gate (MND).
The carbon uptake of the packaging materials is not included Installation into the building (A5)
below as their end-of-life impact is not declared in module A5. The end-of-life impact of the used packaging materials is not
Name Value Unit declared. However, its impact can be modelled based on the
data given below.
Biogenic carbon content in product 286.8 kg C/m³
Stored carbon dioxide in the product 1051.7 kg CO2/m³
5 Environmental Product Declaration - Unilin B.V. Division Panels - Unilin Chipboard
Name Value Unit In module D, the loads and benefits of exporting secondary
material or fuel from the system under study are inventoried.
Wood-based packaging 23.15 kg/m³
The moisture content of this material/fuel is assumed to remain
Cardboard 0.23 kg/m³
at a total of 6 %. This value may vary significantly based on the
PET straps 0.18 kg/m³
storage conditions prior to its intended use.
Stretch foil 0.05 kg/m³
Recycling (secondary material)
Information on the reference lifetime can be found in section
To correctly model the recycling potential, the net flow of
2.12. Please contact Unilin's sales team or
secondary material in the system was mapped during the
info.panels@unilin.com for more information.
product's entire lifecycle. It is assumed that post-consumer
End-of-life (C1-C4)
wood chips replace fresh wood chips. The avoided impact of
The following table provides the parameters required to model this fresh wood chips production was thus modeled using
the end-of-life of the product under study. Since the product is secondary data from EcoInvent.
not intended for extended outdoor use, it is assumed that its
moisture content remains consistent with its state at the factory Energy Recovery (secondary fuel)
gate. The end-of-life product reaches its end-of-waste state Similarly, the recovery potential is modeled based on the net
after (preliminary) sorting and shredding. The losses during the output flow of secondary fuel. It is assumed that a biomass
sorting and shredding are assumed to have a negligible impact power plant located in the EU recovers the secondary fuel's
and are thus discarded. The material leaves the system either energy, with 55 % of the energy being recovered as heat and
as secondary material (recycling) or as secondary fuel (energy the remaining 30 % as electricity. The generated energy
recovery). carriers are assumed to substitute heat and electricity in
accordance with the average mix available on the European
Name Value Unit grid.
Collected separately waste type waste type 676 kg Name Value Unit
Secondary material (output at C3) 676 kg/m³ Net output flow of secondary material 145 kg/m³
Secondary fuel (output at C3) 676 kg/m³ Net output flow of secondary fuel 520 kg/m³
Energy Efficiency Biomass plant 85 %
Reuse, recovery and/or recycling potentials (D)
6 Environmental Product Declaration - Unilin B.V. Division Panels - Unilin Chipboard
5. LCA: Results
The declared values refer to 1 m³ of Unilin Chipboard with a sales-weighted average composition and density of 659 kg/m³.
As previously stated, two end-of-life scenarios are evaluated: energy recovery (secondary fuel) and recycling (secondary material).
These scenarios only affect modules C3 and D, thus two sets of impacts for each module are given below. Columns C3/1 and D/1
represent the scenario in which the end-of-life product exits the system as a secondary fuel, while the impacts of the recycling scenario
are described in columns C3/2 and D/2.
Table "Description of the system boundary" summarizes the scope of the system under study from a life cycle point of view. Declared
modules are indicated with an "X", non-declared modules are indicated with "MND". "MNR" refers to modules which are deemed as not
relevant.
DESCRIPTION OF THE SYSTEM BOUNDARY (X = INCLUDED IN LCA; MND = MODULE OR INDICATOR NOT DECLARED; MNR
= MODULE NOT RELEVANT)
Benefits and
Construction loads beyond
Product stage Use stage End of life stage
process stage the system
boundaries
la ire ta m w a Ry lp p u s tro p s n a rT g n iru tc a fu n a M e h t m o rf tro p s n a rTe tis e h t o t e ta g y lb m e s s A e s U e c n a n e tn ia M ria p e R tn e m e c a lp e R tn e m h s ib ru fe R y g re n e la n o ita re p Oe s u re ta w la n o ita re p Oe s u n o itc u rts n o c -e Dn o itilo m e d tro p s n a rT g n is s e c o rp e ts a W la s o p s iD -e s u e R-y re v o c e R-g n ilc y c e Rla itn e to p
A1 A2 A3 A4 A5 B1 B2 B3 B4 B5 B6 B7 C1 C2 C3 C4 D
X X X MND MND MND MND MNR MNR MNR MND MND X X X X X
RESULTS OF THE LCA - ENVIRONMENTAL IMPACT according to EN 15804+A2: 1 m³ Unilin Chipboard
Parameter Unit A1-A3 C1 C2 C3/1 C3/2 C4 D/1 D/2
GWP-total kg CO 2 eq -9.1E+02 0 2.92E+00 1.06E+03 1.06E+03 0 -5.1E+02 -8.9E+00
GWP-fossil kg CO 2 eq 1.41E+02 0 2.92E+00 1.14E+01 1.14E+01 0 -5.09E+02 -8.8E+00
GWP-biogenic kg CO 2 eq -1.05E+03 0 9.46E-04 1.05E+03 1.05E+03 0 -8.76E-01 -4.17E-02
GWP-luluc kg CO 2 eq 2.14E-01 0 1.13E-03 1.55E-02 1.55E-02 0 -7.03E-01 -5.68E-02
ODP kg CFC11 eq 2.75E-05 0 7.33E-07 1.64E-06 1.64E-06 0 -6.61E-05 -1.27E-06
AP mol H+ eq 1.07E+00 0 9.37E-03 6.43E-02 6.43E-02 0 -5.92E-01 -6.85E-02
EP-freshwater kg P eq 3.75E-03 0 2.1E-05 6.27E-04 6.27E-04 0 -3.08E-02 -7.43E-04
EP-marine kg N eq 2.64E-01 0 2.06E-03 1.64E-02 1.64E-02 0 3.4E-01 -2.14E-02
EP-terrestrial mol N eq 3.41E+00 0 2.29E-02 1.83E-01 1.83E-01 0 3.72E+00 -2.42E-01
kg NMVOC
POCP 8.06E-01 0 9.02E-03 5.19E-02 5.19E-02 0 6.91E-01 -7.5E-02
eq
ADPE kg Sb eq 1.32E-03 0 7.26E-06 3.8E-05 3.8E-05 0 -1.56E-04 -5.81E-05
ADPF MJ 3.09E+03 0 4.78E+01 2.07E+02 2.07E+02 0 -1.21E+04 -1.64E+02
m3 world eq
WDP 1.41E+02 0 1.62E-01 5.74E-01 5.74E-01 0 -6.69E+01 -6.73E+00
deprived
GWP = Global warming potential; ODP = Depletion potential of the stratospheric ozone layer; AP = Acidification potential of land and water; EP =
Eutrophication potential; POCP = Formation potential of tropospheric ozone photochemical oxidants; ADPE = Abiotic depletion potential for non-fossil
resources; ADPF = Abiotic depletion potential for fossil resources; WDP = Water (user) deprivation potential)
RESULTS OF THE LCA - INDICATORS TO DESCRIBE RESOURCE USE according to EN 15804+A2: 1 m³ Unilin Chipboard
Parameter Unit A1-A3 C1 C2 C3/1 C3/2 C4 D/1 D/2
PERE MJ 1.95E+03 0 6.09E-01 1.05E+04 1.05E+04 0 -9.93E+02 -9.01E+02
PERM MJ 1.05E+04 0 0 -1.05E+04 -1.05E+04 0 0 2.25E+03
PERT MJ 1.25E+04 0 6.09E-01 2.19E+01 2.19E+01 0 -9.93E+02 1.35E+03
PENRE MJ 1.86E+03 0 4.78E+01 1.43E+03 1.43E+03 0 -1.21E+04 -1.64E+02
PENRM MJ 1.26E+03 0 0 -1.22E+03 -1.22E+03 0 0 2.61E+02
PENRT MJ 3.12E+03 0 4.78E+01 2.07E+02 2.07E+02 0 -1.21E+04 9.7E+01
SM kg 5.58E+02 0 0 0 0 0 0 1.45E+02
RSF MJ 1.2E+03 0 0 0 0 0 6.88E+03 0
NRSF MJ 0 0 0 0 0 0 7.96E+02 0
FW m3 4.09E+00 0 5.69E-03 1.15E-01 1.15E-01 0 -4.9E+00 -2.07E-01
PERE = Use of renewable primary energy excluding renewable primary energy resources used as raw materials; PERM = Use of renewable primary
energy resources used as raw materials; PERT = Total use of renewable primary energy resources; PENRE = Use of non-renewable primary energy
excluding non-renewable primary energy resources used as raw materials; PENRM = Use of non-renewable primary energy resources used as raw
materials; PENRT = Total use of non-renewable primary energy resources; SM = Use of secondary material; RSF = Use of renewable secondary fuels;
NRSF = Use of non-renewable secondary fuels; FW = Use of net fresh water
RESULTS OF THE LCA – WASTE CATEGORIES AND OUTPUT FLOWS according to EN 15804+A2:
1 m³ Unilin Chipboard
Parameter Unit A1-A3 C1 C2 C3/1 C3/2 C4 D/1 D/2
7 Environmental Product Declaration - Unilin B.V. Division Panels - Unilin Chipboard
HWD kg 1.3E+01 0 3.31E-02 3.08E-01 3.08E-01 0 -2.28E+00 -2.64E-01
NHWD kg 6.38E+01 0 4.72E+00 8.46E+00 8.46E+00 0 -7.37E+01 -5.11E+00
RWD kg 6.26E-03 0 3.24E-04 1.44E-03 1.44E-03 0 -4.81E-02 -8.75E-04
CRU kg 0 0 0 0 0 0 0 0
MFR kg 0 0 0 0 6.76E+02 0 0 0
MER kg 0 0 0 6.76E+02 0 0 0 0
EEE MJ 0 0 0 0 0 0 0 0
EET MJ 0 0 0 0 0 0 0 0
HWD = Hazardous waste disposed; NHWD = Non-hazardous waste disposed; RWD = Radioactive waste disposed; CRU = Components for re-use;
MFR = Materials for recycling; MER = Materials for energy recovery; EEE = Exported electrical energy; EET = Exported thermal energy
RESULTS OF THE LCA – additional impact categories according to EN 15804+A2-optional:
1 m³ Unilin Chipboard
Parameter Unit A1-A3 C1 C2 C3/1 C3/2 C4 D/1 D/2
Disease
PM 1.19E-05 0 3.41E-07 7.57E-07 7.57E-07 0 7.54E-06 -2.5E-06
incidence
IR kBq U235 eq 5.56E+00 0 2.07E-01 1.41E+00 1.41E+00 0 -5.53E+01 -8.48E-01
ETP-fw CTUe 4.73E-05 0 5.86E-08 2.88E-07 2.88E-07 0 -1.39E-06 -1.87E-04
HTP-c CTUh 4.26E-07 0 4.76E-10 3.2E-09 3.2E-09 0 2.6E-08 -3.28E-08
HTP-nc CTUh 7.79E-08 0 1.33E-09 1.05E-08 1.05E-08 0 -5.6E-08 -7.4E-09
SQP SQP 1.3E+04 0 5.47E+01 1.01E+02 1.01E+02 0 -9.47E+02 -4.92E+03
PM = Potential incidence of disease due to PM emissions; IR = Potential Human exposure efficiency relative to U235; ETP-fw = Potential comparative
Toxic Unit for ecosystems; HTP-c = Potential comparative Toxic Unit for humans (cancerogenic); HTP-nc = Potential comparative Toxic Unit for humans
(not cancerogenic); SQP = Potential soil quality index
Disclaimer 1 – for the indicator “Potential Human exposure efficiency relative to U235”. This impact category deals mainly with the
eventual impact of low-dose ionizing radiation on human health of the nuclear fuel cycle. It does not consider effects due to possible
nuclear accidents, occupational exposure or radioactive waste disposal in underground facilities. Potential ionizing radiation from the
soil, radon and from some construction materials is also not measured by this indicator.
Disclaimer 2 – for the indicators “abiotic depletion potential for non-fossil resources”, “abiotic depletion potential for fossil resources”,
“water (user) deprivation potential, deprivation-weighted water consumption”, “potential comparative toxic unit for ecosystems”,
“potential comparative toxic unit for humans – cancerogenic”, “Potential comparative toxic unit for humans - not cancerogenic”,
“potential soil quality index”. The results of this environmental impact indicator shall be used with care as the uncertainties on these
results are high as there is limited experience with the indicator.
6. LCA: Interpretation
This section aims to analyze and interpret the results of the During its growth, wood absorbs CO through photosynthesis
2
LCA analysis carried for 1 m³ of the Unilin Chipboard. The and stores it as biogenic carbon in its biomass. The chipboard's
results shown below, for both end-of-life scenario's, refer to the high wood content results in a GWP-total of - 910 kg/m³. The
product with a sales-weighted average composition. Although product thus stores carbon and does not contribute to global
the values for specific commercial references can vary from the warming when it leaves Unilin's factory gate. The stored carbon
declared and discussed ones, the observed trends will be the will only be released if the chipboard can no longer fulfill its
same throughout the entire product category. intended purpose (end of life).
Summary A deep dive in the drivers of the cradle-to-gate environmental
impact shows the significant contribution of the raw materials
This part intends to summarize the trends observed in the (module A1). 53 % of the fossil CO emissions can primarily be
2
cradle-to-gate environmental impact of the Unilin Chipboard. An
allocated to the (M)UF-glue production, as well as 98 % of the
in-depth analysis is available in the following subsections.
water used in A1 - A3. The generation of heat and electricity,
required for the chipboard's production, is an important driver of
Unilin Chipboard is composed of 85 % wood, of which 92 % is
the production-related impact. This is observable in the AP, EP,
pre- and post-consumer recycled wood. This is highlighted in
POCP indicators.
the 'use of secondary material' indicator, which has a value of
558 kg SM/m³ chipboard for modules A1 - A3.
8 Environmental Product Declaration - Unilin B.V. Division Panels - Unilin Chipboard
Energy Recovery (Secondary Fuel) The GWP-focused analysis also illustrates the "avoided" impact
(described in module D) related to the export of end-of-life
The hot-spot analysis highlights the negative GWP-value of chipboard as a secondary fuel. The energy recovery of the
modules A1 - A3, as depicted in the GWP-focused one. To secondary fuel generates heat and electricity, which substitutes
improve the clarity of the graph, the values of the GWP-luluc a European averaged mix of heat and electricity from the grid.
indicator have been omitted. Since the largest share of the heat and electricity on the
European grid is fossil-based, a negative GWP-fossil is
Wood stores CO as biogenic carbon during its growth (GWP- obtained (i.e. avoided fossil CO emissions from combustion). It
2 2
biogenic = -1051 kg CO eq./m³). This negative GWP-value is indicates that the combustion of these fossil fuels has a higher
2
partially counterbalanced by the positive GWP-impact of the impact on global warming than the energy recovery from the
fossil materials and energy resources used during A1 - A3 secondary fuel.
(GWP-fossil). This results in a GWP-total of - 910 kg CO
2
eq./m³ when the Unilin Chipboard leaves the factory gate. The
The hot-spot analysis shows that, for non-GWP-related
product under study thus stores carbon and does not contribute
parameters, modules A1 - A3 are the main contributors to the
to the global warming potential.
system under study. Values for module D are generally
negative, except for the EP and POCP indicators. This is
The stored carbon will only be released when the end-of-life
attributed to the emissions from the energy recovery process of
product leaves the system as a secondary fuel. The figure
the end-of-life chipboard.
below clearly demonstrates a neutral biogenic carbon balance
in accordance with EN16485.
9 Environmental Product Declaration - Unilin B.V. Division Panels - Unilin Chipboard
accommodates the transfer of the wood's biogenic carbon
Recycling (Secondary Material) content from the system under study to a subsequent system. It
is assumed that the exported secondary material replaces fresh
If the end-of-life chipboard leaves the system as a secondary wood chips.
material, the cradle-to-gate environmental impact remains the
same as for the energy recovery scenario. The end-of-waste The non-GWP-related parameters show a lower contribution of
state is achieved (for both secondary material and fuel) after module D to the core environmental indicators in comparison to
sorting and shredding the end-of life chipboard. The the energy recovery EOL scenario. This is attributed to the fact
environmental impact during module C3 also remains the that the production of wood chips from fresh wood is less
same. The GWP-focused hot-spot analysis, shown below, also environmentally encumbered than the combustion processes
demonstrates a neutral biogenic carbon balance over the needed to generate (fossil-based) energy carriers.
chipboard's entire life cycle. This carbon balance
10 Environmental Product Declaration - Unilin B.V. Division Panels - Unilin Chipboard
WDP. 98 % of all water used in modules A1 - A3 is allocated to
Product Stage (A1 - A3) - Main Drivers the production of the raw materials (mainly related to the
production of (M)UF-glue).
The graph below allows to identify the primary sources of the
cradle-to-gate environmental impact. The results show that raw Energy-related processes are typically the main drivers of the
material production (module A1) has a significant impact. 53 % environmental impact of module A3. This is observed in the
of the fossil CO emissions are primarily attributed to the contribution of A3 to AP, EP and POCP, which is traced back to
2
production of (M)-UF glue. The contribution of the raw material the generation of electricity and heat at the adjacent biomass
production is even more significant for the indicators ADPE and plants A&S and A&U.
7. Requisite evidence
Formaldehyde emissions
• Test report : 230061-REQ1
E1 - EN 13986:2004+A1:2015
• Method : ASTM D6007-14
• Test report : QA-2023-0135 • Product : Belspan LF
• Method : EN ISO 12460-5 • Laboratory : Wood.be
• Product : Belspan LF+ • Result : 0.05 ppm [Limit value < 0.09 ppm]
• Laboratory : WKI Fraunhofer
• Result : 2.3 mg/100g DS [Limit value < 8 mg/100g DS) PCP + Heavy metals + Wood preservative analysis
• Test Report : 0001131684/20 AZ 593092
E0.5 - ChemVerbotsV
• Method : see report details
• Test report : QA-2023-0134 • Product : Belspan LF+
• Method : EN 717-1 • Laboratory : TUV Reinland
• Product : Belspan LF+ • Result : PCP < 0.1 mg/kg; Lindane < 0.1 mg/kg; Lead
• Laboratory : WKI Fraunhofer 67 mg/kg; Arsenic < 5 mg/kg; Chromium < 10 mg/kg;
• Result : 0.03 ppm [Limit value < 0.05 ppm) Copper 11 mg/kg
.
CARB2/TSCA Title VI
11 Environmental Product Declaration - Unilin B.V. Division Panels - Unilin Chipboard
VOC Emissions finish in their end application. The type of finish (melamine,
paper foil, veneer, HPL,...) will determine the indoor air quality.
Unspecified while raw chipboards are always coated with a
8. References
Standards EN 15804
ASTM D6007 EN 15804:2012+A2:2019+AC:2021, Sustainability of
construction works — Environmental Product Declarations —
ASTM D6007:2020, Standard Test Method for Determining Core rules for the product category of construction products.
Formaldehyde Concentrations in Air from Wood Products Using
a Small-Scale Chamber. EN 16368
ASTM E1333 EN 16368:2014, Lightweight Particleboards –Specifications.
ASTM E1333:2020, Standard Test Method for Determining EN 16449
Formaldehyde Concentrations in Air and Emission Rates from
Wood Products Using a Large Chamber. EN 16449:2014, Wood and wood-based produts - Calculation
of the biogenic carbon content of wood and conversion to
EN 310 carbon dioxide.
EN 310:1993, Wood-based panels - Determination of modulus EN 16485
of elasticity in bending and of bending strength.
EN 16485:2014, Round and sawn timber. Environmental
EN 312 Product Declarations. Product category rules for wood and
wood-based products for use in construction.
EN 312:2010-12, Particleboards – Specifications
EN 16516
EN 319
EN 16516:2020, Construction products: Assessment of release
EN 319:1993, Particleboards and fibreboards - Determination of dangerous substances - Determination of emissions into
of tensile strength perpendicular to the plane of the board indoor air.
EN 322 ISO 9001
EN 322:1993, Wood-based panels - Determination of moisture EN ISO 9001:2008-11, Quality Management Systems –
content Requirements.
EN 323 ISO 14025
EN 323:2005, Wood-based panels - Determination of density. EN ISO 14025:2011, Environmental labels and declarations —
Type III environmental declarations — Principles and
EN 717-1 procedures.
EN 717-1:2004, Wood-based panels - Determination of ISO 14040
formaldehyde release Formaldehyde emission by the chamber
method. EN ISO 14040:2006-10, Environmental management — Life
cycle assessment — Principles and framework.
EN 12460-5
ISO 14044
EN 12460-5:2015, Wood-based panels. Determination of
formaldehyde release Extraction method (called the perforator ISO 14044:2006-10, Environmental management — Life cycle
method). assessment — Principles and framework.
EN 13501-1 JIS A 1460
EN 13501-1:2007-05+A1:2009, Fire classification of JIS A 1460:2021, Building boards Determination of
construction products and building elements - Part 1: formaldehyde emission -- Desiccator method.
classification with the results of tests on the reaction to fire of
building products. JIS A 5908
EN 13986 JIS A 5908:2022, Particleboards
EN 13986:2004+A1:2015, Wood-based panels for use in
construction— Characteristics, valuation of conformity and
marking.
12 Environmental Product Declaration - Unilin B.V. Division Panels - Unilin Chipboard
Additional References Federal Official Journal I 2001, 3379.
BBSR Table IBU 2022
BBSR 2017, Useful lives of building components for life cycle Institut Bauen und Umwelt e.V.: General Instructions for the
analyses according to the Sustainable Building Assessment EPD programme of Institut Bauen und Umwelt e.V., Version
System, 2017, BBSR Germany 2017. 2.1, Berlin: Institut Bauen und Umwelt e.V., 2022
www.ibu-epd.com
CPR
PCR Part A
CPR EU Ordinance No. 305/2011 of the European Parliament
and Council of 9th March 2011 to define harmonized conditions Product Category Rules for Building-Related Products and
for marketing building products. Services. Part A: Calculation Rules for the Life Cycle
Assessment and Requirements on the Project Report according
EcoInvent 3.8. to EN 15804+A2:2019. Version 1.3. Berlin: Institut Bauen und
Umwelt e.V. (eds.), 2021.
Ecoinvent 3.8, Database for Life Cycle Inventory and
Assessment. Swiss Centre for Life Cycle Inventories, 2021. PCR Part B
Available at: https://ecoinvent.org/the-ecoinvent-database/data-
releases/ecoinvent-3-8/. Product Category Rules for Building-Related Products and
Services. Part B: Requirements on the EPD for Wood based
EU Biocidal Products Ordinance No. 528/2012 panels. Version 2. Berlin: Institut Bauen und Umwelt e.V. (eds.),
2023.
Regulation (EU) No 528/2012 of the European Parliament and
Council of 22 May 2012 concerning the making available on the SVHC List
market and use of biocidal products.
List of Substances of Very High Concern (SVHC) Candidate for
EWC Authorisation (ECHA Candidate List), dated 04.07.2023,
published in accordance with Article 59(10) of the REACH
European Waste Catalogue, Ordinance on the European Waste Regulation. Helsinki: European Chemicals Agency.
Catalogue (Waste Catalogue Ordinance - AVV), reference
13 Environmental Product Declaration - Unilin B.V. Division Panels - Unilin Chipboard
Publisher
Institut Bauen und Umwelt e.V. +49 (0)30 3087748- 0
Hegelplatz 1 info@ibu-epd.com
10117 Berlin www.ibu-epd.com
Germany
Programme holder
Institut Bauen und Umwelt e.V. +49 (0)30 3087748- 0
Hegelplatz 1 info@ibu-epd.com
10117 Berlin www.ibu-epd.com
Germany
Author of the Life Cycle Assessment
Unilin B.V. Division Panels +32 56 67 52 11
Ooigemstraat 3 info.panels@unilin.com
8710 Wielsbeke https://www.unilinpanels.com/en-
Belgium gb
Owner of the Declaration
Unilin B.V. Division Panels +32 56 66 70 21
Ooigemstraat 3 info.panels@unilin.com
8710 Wielsbeke https://www.unilinpanels.com/en-
Belgium gb
14 Environmental Product Declaration - Unilin B.V. Division Panels - Unilin Chipboard
