ENVIRONMENTAL PRODUCT DECLARATION
as per ISO 14025 and EN 15804+A2
Owner of the Declaration dormakaba International Holding GmbH
Publisher Institut Bauen und Umwelt e.V. (IBU)
Programme holder Institut Bauen und Umwelt e.V. (IBU)
Declaration number EPD-DOR-20220217-CBA1-EN
Issue date 29.11.2022
Valid to 28.11.2027
ESA 400 Automatic Sliding Door
Dormakaba
www.ibu-epd.com | https://epd-online.com
General Information
Dormakaba ESA 400 Automatic Sliding Door
Programme holder Owner of the declaration
IBU – Institut Bauen und Umwelt e.V. dormakaba International Holding GmbH
Hegelplatz 1 DORMA Platz 1
10117 Berlin 58256 Ennepetal
Germany Germany
Declaration number Declared product / declared unit
EPD-DOR-20220217-CBA1-EN 1 piece of the product: Automatic sliding door ESA 400 consisting of the
following items:
- header
- drive
- panels and jambs
- glass
- packaging material
This declaration is based on the product category rules: Scope:
Automatic doors, automatic gates, and revolving door systems, This EPD refers to a specific automatic sliding door ESA 400 produced by
01.08.2021 dormakaba USA Inc. The production site is located in Reamstown, PA
(PCR checked and approved by the SVR) USA.
The year of data collection is 2022.
Issue date The owner of the declaration shall be liable for the underlying information
and evidence; the IBU shall not be liable with respect to manufacturer
29.11.2022
information, life cycle assessment data and evidences.
The EPD was created according to the specifications of EN 15804+A2. In
Valid to
the following, the standard will be simplified as EN 15804.
28.11.2027
Verification
The standard EN 15804 serves as the core PCR
Independent verification of the declaration and data according to ISO
14025:2011
internally X externally
Dipl.-Ing. Hans Peters
(Chairman of Institut Bauen und Umwelt e.V.)
Florian Pronold Dr.-Ing. Wolfram Trinius,
(Managing Director Institut Bauen und Umwelt e.V.) (Independent verifier)
1 Environmental Product Declaration - Dormakaba - ESA 400 Automatic Sliding Door
Product
Delivery status:The delivery status of an average ESA 400
Product description/Product definition automatic sliding door includes header, drive, panels, jambs,
The ESA 400 Fine Frame Automatic Sliding Door is elegant and glass and packaging materials:
upscale; perfect marriage of beauty and functionality.
Recommended for standard openings for office and apartment
building applications. Full breakout provides enhanced egress
capacity.
Features
• Breakout of sliding panels and sidelite
Base materials/Ancillary materials
• All Glass Look
The ESA 400 automatic sliding door fine frame comprises the
• Dual Vertical Weather Sweeps
following components:
• Factory Glazed 3/8' tempered glass
• Heavy-duty Delrin® and Brass Rollers
• Fully monitored overhead presence and activation
sensors
• Security interface
• Low maintenance
• High traffic volume
• Adjustable astragal
Optional Features
• Battery backup for keeping the door operational during
power loss
• Various thresholds to fit any site condition
• Transom
• Crash bars
• Glass stops up to 1"; sloped glass stops available
The product contains partial articles which contain substances
For placing on the market following standards are applicable:
listed in the Candidate List of REACH Regulation
• EN 16005 1907/2006/EC (date: 10.06.2022) exceeding 0.1 percentage by
• ICC/IBC International Building Code mass: no
• ANSI/BHMA A 156.10 American National Standard for
Power Operated Doors Pedestrian Doors Reference service life
• UL 325 Listed The life cycle of the ESA 400 door system is about 10 years,
• NFPA 70 National Electrical Code depending on the application and frequency of use. Regular
• NFPA 101 Life Safety Code maintenance is advised to ensure a life expectancy of 10 years.
• CUL Approved for use in Canada For repairs or renewals, suitable spare parts are available. The
drive is tested to 1,000,000 closing cycles according to EN
Application 16005.
Recommended for standard openings for office and apartment
building applications. Full breakout provides enhanced egress
capacity.
Technical Data
The technical specification of the ESA 400 is as follows:
Constructional data
Name Value Unit
Height 240 mm
Installation depth 152 mm
Opening speed maximum 50 cm/s
Closing speed maximum 40 cm/s
Hold open time maximum 60 s
Supply voltage, frequency maximum 60 Hz
Power supply maximum 60 Hz
Internal power available 27 VDC/2A
Fuse 6.6 A
Power consumption maximum 250 W
LCA: Calculation rules
Declared unit
Declared Unit
The declared unit is 1 piece of the product: ESA 400 Automatic Name Value Unit
Sliding Door Declared unit 1 pce.
Mass (total system) 217,70 kg
2 Environmental Product Declaration - Dormakaba - ESA 400 Automatic Sliding Door
End-of-life stage– Modules C1-C4 and D
System boundary The end-of-life stage includes:
The type of EPD is: cradle-to-gate with options, modules C1– — C1, de-construction, demolition:
C4, and module D (A1–A3 + C + D and additional modules: A4 — C2, transport to waste processing;
+ A5 + B6) — C3, waste processing for reuse, recovery and/or recycling;
— C4, disposal;
Production - Module A1-A3 including provision and all transport, provision of all materials,
The product stage includes: products and related energy and water use.
— A1, raw material extraction, processing and mechanical
treatments, processing of secondary material input (e.g.
recycling processes), — A2, transport to the manufacturer, Module D (Benefits and loads beyond the system boundary)
— A3, manufacturing and assembly including provision of all includes:
materials, products and energy, as well as waste processing up — D, recycling potentials, expressed as net impacts and
to the end-of-waste state. benefits.
Construction stage - Modules A4-A5 Geographic Representativeness
The construction process stage includes: Land or region, in which the declared product system is
— A4, transport to the building site; manufactured, used or handled at the end of the product´s
— A5, installation into the building; lifespan: Global
including provision of all materials, products and energy, as well
as waste processing up to the end-of waste state or disposal of
Comparability
final residues during the construction process stage.
Basically, a comparison or an evaluation of EPD data is only
Use stage - Module B6 possible if all the data sets to be compared were created
The use stage related to the operation of the building includes: according to EN 15804 and the building context, respectively
— B6, operational energy use the product-specific characteristics of performance, are taken
into account. Background database: GaBi, SP40.
LCA: Scenarios and additional technical information
Characteristic product properties of biogenic carbon
Information on describing the Biogenic Carbon Content at Operational energy use (B6)
factory gate The use stage is declared for 10 years
Name ValueUnit Name Value Unit
Biogenic carbon content in product 0.25 kg Electricity consumption for 1 year 189.29 kWh
C
Days per year in use 365 days
Biogenic carbon content in accompanying kg
0.74 On mode per day 1.8 h
packaging C
Idle mode per day 22.2 h
Note: 1 kg of biogenic carbon is equivalent to 44/12 kg of CO .
2 On mode power 14,31 W
Idle mode power 22.2 W
The following technical scenario information is required for the End of life (C1-C4)
declared modules
Name Value Unit
Transport from the gate to the site (A4)
Collected separately waste type 214.7 kg
Name Value Unit Recycling 100 kg
Litres of fuel (per 1 kg) 0.00276 l/100km Energy recovery 0.7 kg
Capacity utilisation (including empty runs) 55 % Landfilling 114 kg
Transport distance via medium truck 100 km Transport to waste management 50 km
Transport distance is declared for a distance of 100km by truck The product is disassembled in a recycling process.
in order to allow scaling to a specific point of installation. Material recycling is then assumed for the metals and
electronics. The plastic components are assumed to be
Installation into the building (A5) incinerated with energy recovery. Glass, electromechanics and
minor proportions of residues arising from the recycling process
Name Value Unit
are landfilled.
Waste packaging (paper and plastic) 3 kg
Region for the End of Life is: Global.
Reference service life
Reuse, recovery and/or recycling potentials (D),
Name Value Unit
relevant scenario information
Life Span according to the manufacturer 10 a The collection rate is 100 %.
3 Environmental Product Declaration - Dormakaba - ESA 400 Automatic Sliding Door
LCA: Results
DESCRIPTION OF THE SYSTEM BOUNDARY (X = INCLUDED IN LCA; MND = MODULE OR INDICATOR NOT DECLARED; MNR
= MODULE NOT RELEVANT)
Benefits and
Construction loads beyond
Product stage Use stage End of life stage
process stage the system
boundaries
la ire ta m w a Ry lp p u s tro p s n a rT g n iru tc a fu n a M e h t m o rf tro p s n a rTe tis e h t o t e ta g y lb m e s s A e s U e c n a n e tn ia M ria p e R tn e m e c a lp e R tn e m h s ib ru fe R y g re n e la n o ita re p Oe s u re ta w la n o ita re p Oe s u n o itc u rts n o c -e Dn o itilo m e d tro p s n a rT g n is s e c o rp e ts a W la s o p s iD -e s u e R-y re v o c e R-g n ilc y c e Rla itn e to p
A1 A2 A3 A4 A5 B1 B2 B3 B4 B5 B6 B7 C1 C2 C3 C4 D
X X X X X MND X MNR MNR MNR X MND X X X X X
RESULTS OF THE LCA - ENVIRONMENTAL IMPACT according to EN 15804+A2: 1 piece ESA 400 Automatic Sliding Door
Parameter Unit A1-A3 A4 A5 B2 B6 C1 C2 C3 C4 D
GWP-total kg CO 2 eq 1.04E+03 1.9E+00 5.38E+00 0 1.06E+03 0 9.39E-01 4.04E+00 1.74E+00 -5.34E+02
GWP-fossil kg CO 2 eq 1.04E+03 1.82E+00 2.61E+00 0 1.06E+03 0 8.97E-01 2.42E+00 1.72E+00 -5.32E+02
GWP-
biogenic kg CO 2 eq -3.15E+00 8.4E-02 2.77E+00 0 2.3E-01 0 4.1E-02 1.62E+00 6E-03 -1.72E+00
GWP-luluc kg CO 2 eq 6.79E-01 4.33E-05 1.9E-04 0 3.21E-01 0 2.14E-05 1.45E-04 5E-03 -7.9E-02
ODP kg CFC11 eq 1.09E-09 1.92E-16 1.79E-15 0 3.74E-12 0 9.47E-17 1.33E-15 6.39E-15 -4.36E-09
AP mol H+ eq 5.48E+00 2E-03 1E-03 0 1.72E+00 0 8.98E-04 5.91E-04 1.2E-02 -2.04E+00
EP-
kg P eq 1.08E-03 3.9E-07 3.04E-07 0 5.81E-04 0 1.92E-07 2.11E-07 2.96E-06 -2.63E-04
freshwater
EP-marine kg N eq 8.71E-01 5.8E-04 3.89E-04 0 3.68E-01 0 2.86E-04 1.34E-04 3E-03 -2.65E-01
EP-terrestrial mol N eq 9.68E+00 6E-03 6E-03 0 3.95E+00 0 3E-03 3E-03 3.5E-02 -2.88E+00
kg NMVOC
POCP 2.37E+00 2E-03 1E-03 0 1.05E+00 0 8.08E-04 3.76E-04 1E-02 -8.37E-01
eq
ADPE kg Sb eq 4.43E-03 5.46E-08 2.57E-08 0 2.11E-04 0 2.69E-08 1.85E-08 1.55E-07 -5.38E-04
ADPF MJ 1.36E+04 2.58E+01 2.07E+00 0 1.72E+04 0 1.27E+01 1.32E+00 2.26E+01 -7.63E+03
m3 world eq
WDP 1.41E+02 4E-03 6.12E-01 0 2.06E+02 0 2E-03 3.91E-01 1.81E-01 -2.35E+01
deprived
GWP = Global warming potential; ODP = Depletion potential of the stratospheric ozone layer; AP = Acidification potential of land and water; EP =
Eutrophication potential; POCP = Formation potential of tropospheric ozone photochemical oxidants; ADPE = Abiotic depletion potential for non-fossil
resources; ADPF = Abiotic depletion potential for fossil resources; WDP = Water (user) deprivation potential)
RESULTS OF THE LCA - INDICATORS TO DESCRIBE RESOURCE USE according to EN 15804+A2: 1 piece ESA 400 Automatic
Sliding Door
Parameter Unit A1-A3 A4 A5 B2 B6 C1 C2 C3 C4 D
PERE MJ 4.75E+03 8.1E-02 2.45E+01 0 2.72E+03 0 4E-02 2.17E+01 2.96E+00 -3.69E+03
PERM MJ 4.54E+01 0 -2.4E+01 0 0 0 0 -2.14E+01 0 0
PERT MJ 4.8E+03 8.1E-02 4.69E-01 0 2.72E+03 0 4E-02 3.29E-01 2.96E+00 -3.69E+03
PENRE MJ 1.36E+04 2.58E+01 4.51E+01 0 1.72E+04 0 1.27E+01 2.48E+01 2.26E+01 -7.63E+03
PENRM MJ 6.65E+01 0 -4.3E+01 0 0 0 0 -2.35E+01 0 0
PENRT MJ 1.36E+04 2.58E+01 2.07E+00 0 1.72E+04 0 1.27E+01 1.32E+00 2.26E+01 -7.63E+03
SM kg 6.75E+00 0 0 0 0 0 0 0 0 0
RSF MJ 0 0 0 0 0 0 0 0 0 0
NRSF MJ 0 0 0 0 0 0 0 0 0 0
FW m3 1.19E+01 1.46E-04 1.4E-02 0 6.3E+00 0 7.2E-05 9E-03 6E-03 -6.42E+00
PERE = Use of renewable primary energy excluding renewable primary energy resources used as raw materials; PERM = Use of renewable primary
energy resources used as raw materials; PERT = Total use of renewable primary energy resources; PENRE = Use of non-renewable primary energy
excluding non-renewable primary energy resources used as raw materials; PENRM = Use of non-renewable primary energy resources used as raw
materials; PENRT = Total use of non-renewable primary energy resources; SM = Use of secondary material; RSF = Use of renewable secondary fuels;
NRSF = Use of non-renewable secondary fuels; FW = Use of net fresh water
RESULTS OF THE LCA – WASTE CATEGORIES AND OUTPUT FLOWS according to EN 15804+A2:
1 piece ESA 400 Automatic Sliding Door
Parameter Unit A1-A3 A4 A5 B2 B6 C1 C2 C3 C4 D
HWD kg 1.82E-05 2.51E-09 5.81E-09 0 6.63E-06 0 1.24E-09 4.39E-09 3.45E-07 -1.29E-05
NHWD kg 2.45E+02 3E-03 3.53E-01 0 5.35E+00 0 1E-03 2.57E-01 1.14E+02 -1.45E+02
RWD kg 7.19E-01 2.77E-05 9.08E-05 0 1.53E+00 0 1.37E-05 5.35E-05 2.58E-04 -8.72E-01
CRU kg 0 0 0 0 0 0 0 0 0 0
MFR kg 0 0 0 0 0 0 0 1E+02 0 0
MER kg 0 0 0 0 0 0 0 0 0 0
EEE MJ 0 0 9E+00 0 0 0 0 0 0 0
4 Environmental Product Declaration - Dormakaba - ESA 400 Automatic Sliding Door
EET MJ 0 0 1.86E+01 0 0 0 0 0 0 0
HWD = Hazardous waste disposed; NHWD = Non-hazardous waste disposed; RWD = Radioactive waste disposed; CRU = Components for re-use;
MFR = Materials for recycling; MER = Materials for energy recovery; EEE = Exported electrical energy; EET = Exported thermal energy
RESULTS OF THE LCA – additional impact categories according to EN 15804+A2-optional:
1 piece ESA 400 Automatic Sliding Door
Parameter Unit A1-A3 A4 A5 B2 B6 C1 C2 C3 C4 D
Disease
PM 5.08E-05 9.58E-09 1.02E-08 0 1.54E-05 0 4.72E-09 6.4E-09 1.53E-07 -3.31E-05
incidence
IR kBq U235 eq 1.4E+02 4E-03 1.1E-02 0 1.27E+02 0 2E-03 6E-03 2.6E-02 -1.77E+02
ETP-fw CTUe 7.51E+03 1.83E+01 8.67E-01 0 5.13E+03 0 9.02E+00 5.12E-01 1.29E+01 -2.9E+03
HTP-c CTUh 6.42E-07 3.44E-10 6.08E-11 0 1.1E-07 0 1.7E-10 4.59E-11 1.92E-09 -1.4E-07
HTP-nc CTUh 1.16E-05 1.47E-08 4.85E-09 0 4.17E-06 0 7.26E-09 3.98E-09 2.11E-07 -3.89E-06
SQP SQP 1.61E+03 6.6E-02 5.9E-01 0 1.57E+03 0 3.3E-02 3.93E-01 4.72E+00 -2.11E+02
PM = Potential incidence of disease due to PM emissions; IR = Potential Human exposure efficiency relative to U235; ETP-fw = Potential comparative
Toxic Unit for ecosystems; HTP-c = Potential comparative Toxic Unit for humans (cancerogenic); HTP-nc = Potential comparative Toxic Unit for humans
(not cancerogenic); SQP = Potential soil quality index
Disclaimer 1 – for the indicator IRP
This impact category deals mainly with the eventual impact of low dose ionizing radiation on human health of the nuclear fuel cycle. It
does not consider effects due to possible nuclear accidents, occupational exposure nor radioactive waste disposal in underground
facilities. Potential ionizing radiation from the soil, from radon and from some construction materials is also not measured by this
indicator.
Disclaimer 2 – for the indicators ADPE, ADPF, WDP, ETP-fw, HTP-c, HTP-nc, SQP
The results of this environmental impact indicator shall be used with care as the uncertainties on these results are high or as there is
limited experience with the indicator.
References
Standards EN 16005
DIN EN 16005: 2013-01, Power operated pedestrian doorsets -
A156.10 Safety in use - Requirements and test methods.
ANSI A156 - 2017 Power Operated Pedestrian Doors.
ICC/IBC
DIN 18650 The International Building Code (IBC) is a model building code
DIN 18650:2010, Powered pedestrian doors - Product developed by the International Code Council (ICC).
requirements and test methods.
NFPA 70
DIN EN 60335 National Electrical Code 70.
DIN EN 60335-1, -2-103:2020-08, Household and similar
electrical appliances - Safety - Part 1: General requirements. NFPA 101
Life Safety Code 101.
DIN EN 61000
DIN EN 61000-1-2:2017-07, Electromagnetic compatibility UL 325
(EMC) - Part 1-2: General - Methodology for the achievement of UL 325:2017-05-19 Door, curtain, gate, blind and window
functional safety of electrical and electronic systems including operating devices and installations.
equipment with regard to electromagnetic phenomena.
Further References
DIN EN 61508
DIN EN 61508-2:2011-02, Functional safety of 2011/65/EU ROHS3 Directive
electrical/electronic/programmable electronic safety-related Directive 2011/65/EU of the European Parliament and of the
systems - Part 2: Requirements for Council of 8 June 2011 on the restriction of the use of certain
electrical/electronic/programmable electronic safety-related hazardous substances in electrical and electronic equipment.
systems. IBU 2021
General Instructions for the EPD programme of Institut Bauen
DIN EN ISO 13849 und Umwelt e.V.
DIN EN ISO 13849-1:2021-08, Safety of machinery - Safety- Version 2.0, Berlin: Institut Bauen und Umwelt e.V., 2021.
related parts of control systems - Part 1: General principles for www.ibu-epd.com
design.
GaBi ts software
DIN EN ISO 14025 Sphera Solutions GmbH Gabi Software System and Database
DIN EN ISO 14025:201110, Environmental labels and for Life Cycle Engineering 1992-2020 Version 10.0.0.71
declarations — Type III environmental declarations — University of Stuttgart Leinfelden-Echterdingen
Principles and procedures.
GaBi ts documentation
EN 15804 GaBi life cycle inventory data documentation
EN 15804+A2: 2019+AC:2021, Sustainability of construction (https://www.gabisoftware.
works — Environmental Product Declarations — Core rules for com/support/gabi/gabidatabase- 2020-lci-documentation/).
the product category of construction products.
5 Environmental Product Declaration - Dormakaba - ESA 400 Automatic Sliding Door
and Requirements on the Project Re-port according to EN
LCA-tool dormakaba 15804+A2:2019, Version 1.0, Institut Bauen und Umwelt e.V.,
LCA tool, version ENS Door LCA tool No.: IBU-DOR-202107- www.ibu-epd.com.
LT1-EN
Developed by Sphera Solutions GmbH. PCR Part B
PCR – Part B: Requirements on the EPD for Building Hardware
PCR Part A product, version 1.2, Institut Bauen und Umwelt e.V., www.ibu-
PCR – Part A: Calculation Rules for the Life Cycle Assessment epd.com, 2020.
6 Environmental Product Declaration - Dormakaba - ESA 400 Automatic Sliding Door
Publisher
Institut Bauen und Umwelt e.V. +49 (0)30 3087748- 0
Hegelplatz 1 info@ibu-epd.com
10117 Berlin www.ibu-epd.com
Germany
Programme holder
Institut Bauen und Umwelt e.V. +49 (0)30 3087748- 0
Hegelplatz 1 info@ibu-epd.com
10117 Berlin www.ibu-epd.com
Germany
Author of the Life Cycle Assessment
Sphera Solutions GmbH +49 711 341817-0
Hauptstraße 111- 113 info@sphera.com
70771 Leinfelden-Echterdingen www.sphera.com
Germany
Owner of the Declaration
dormakaba International Holding GmbH +49 2333 793-0
DORMA Platz 1 info.de@dormakaba.com
58256 Ennepetal www.dormakaba.com
Germany
7 Environmental Product Declaration - Dormakaba - ESA 400 Automatic Sliding Door
