ENVIRONMENTAL PRODUCT DECLARATION
as per ISO 14025 and EN 15804+A2
Owner of the Declaration dormakaba International Holding GmbH
Publisher Institut Bauen und Umwelt e.V. (IBU)
Programme holder Institut Bauen und Umwelt e.V. (IBU)
Declaration number EPD-DOR-20210197-CBA2-EN
Issue date 07.10.2021
Valid to 06.10.2026
Extension module 90 43
dormakaba
www.ibu-epd.com | https://epd-online.com
General Information
dormakaba Extension module 90 43
Programme holder Owner of the declaration
IBU – Institut Bauen und Umwelt e.V. dormakaba International Holding GmbH
Hegelplatz 1 DORMA Platz 1
10117 Berlin 58256 Ennepetal
Germany Germany
Declaration number Declared product / declared unit
EPD-DOR-20210197-CBA2-EN 1 piece of the product: Extension module 90 43
This declaration is based on the product category rules: Scope:
Electronic and physical Access Control Systems, 01.08.2021 This EPD refers to a specific product manufactured by dormakaba. The
(PCR checked and approved by the SVR) production site is located in Villingen-Schwenningen (Germany).
The data represents the year 2019.
Issue date The owner of the declaration shall be liable for the underlying information
and evidence; the IBU shall not be liable with respect to manufacturer
07.10.2021
information, life cycle assessment data and evidences.
The EPD was created according to the specifications of EN 15804+A2. In
Valid to
the following, the standard will be simplified as EN 15804.
06.10.2026
Verification
The standard EN 15804 serves as the core PCR
Independent verification of the declaration and data according to ISO
14025:2011
internally X externally
Dipl.-Ing. Hans Peters
(Chairman of Institut Bauen und Umwelt e.V.)
Florian Pronold Dr.-Ing. Wolfram Trinius,
(Managing Director Institut Bauen und Umwelt e.V.) (Independent verifier)
1 Environmental Product Declaration - dormakaba - Extension module 90 43
Product
Interface
Product description/Product definition • proprietary in-line bus to host device
With the extension module 90 43, the standalone remote
reader 91 15 becomes a reader with convenient wireless Peripherals Interface
function. This way, you can program doors from your desk and • Radio Technology: IEEE 802.15.4
benefit from the advantages of a wireless access system. It can • Frequency band: 2400 to 2485.5 MHz (16 channels)
be used for doors where you wish to change access rights
wirelessly. For instance, in a system in which doors have been Power supply
equipped with battery operated standalone components and • via proprietary bus from connected host device
have the wireless function. Here you can integrate the entrance
door reader into the same network and operate all doors Installation
conveniently with the click of a mouse. The extension module • Top hat rails: TH35/(7.5/15)
connects directly to the remote reader 91 15 without additional • Class of protection: IP20
wiring effort. For the placing on the market in the European
Union/European Free Trade Association (EU/EFTA) (with the The product is not harmonised in accordance with the
exception of Switzerland) the following legal provisions apply: Construction Product Regulations (CPR) but in accordance with
• Radio Equipment Directive (RED) other provisions for harmonisation of the EU. Compliance with
• Restriction of Hazardous Substances (RoHS) the European Union Directive and technical specifications:
• EN 50581:2012 • EN 301489-1 V2.2.0 Draft
The CE-marking takes into account the proof of conformity with • EN 301489-17 V3.2.1 Draft
the respective harmonized standards based on the legal • EN 300328 V2.1.1
provisions above. For the application and use the respective • EN 62311:2008
national provisions apply. • EN 62368-1:2014-08
The product is subject to CE marking according to the relevant
Application
harmonization legislation.
Wireless access control
It provides a wireless access point for almost any door: Base materials/Ancillary materials
• Standalone systems: as a CardLink update point The major material compositions of the product are listed
• External doors and gates below:
• Automatic doors Name Value Unit
• Parking barriers Paper 45 %
• Entrance areas
Plastics 29 %
• Motor locks
Electronics 25 %
Technical Data Steel <1 %
The extension module 90 43 has the following technical
The product includes partial articles which contain substances
properties:
listed in the Candidate List of REACH Regulation
Name Value Unit 1907/2006/EC (date: 08.07.2021) exceeding 0.1 percentage by
Operating Temperature 0 - 50 °C mass: no
Operating Humidity 5 - 85 %
The Candidate List can be found on the ECHA website
Width Dimension 70 mm
address: https:echa.europa.eu/de/home.
Height Dimension 87 mm
Depth Dimension 45 mm Reference service life
Weight (without packaging) 0,09 kg The reference service life of the dormakaba extension module
Weight (with packaging) 0,145 kg 90 43 is estimated to be 12 years. This number is based on the
support and service life and is not an estimated lifetime.
Power consumption "on mode" 5 W
Power consumption "idle mode" 2 W
LCA: Calculation rules
+ A5 + B6)
Declared Unit
The declared unit is 1 piece of the product: Extension module Production - Module A1-A3
90 43. The product stage includes:
Declared unit — A1, raw material extraction, processing and mechanical
treatments, processing of secondary material input (e.g.
Name Value Unit
recycling processes),
Declared unit 1 pce.
— A2, transport to the manufacturer,
Conversion factor to 1 kg (kg per declared unit) 6.89 - — A3, manufacturing and assembly including provision of all
Product weight including packaging 0,145 kg materials, products and energy, as well as waste processing up
to the end-of waste state.
System boundary
Construction stage - Modules A4-A5
The type of EPD is: cradle to gate with options, modules C1–
The construction process stage includes:
C4, and module D (A1–A3 + C + D and additional modules: A4
2 Environmental Product Declaration - dormakaba - Extension module 90 43
— A4, transport to the building site;
— A5, installation into the building; Module D (Benefits and loads beyond the system boundary)
including provision of all materials, products and energy, as well includes:
as waste processing up to the end-of-waste state or disposal of — D, recycling potentials, expressed as net impacts and
final residues during the construction process stage. benefits.
Use stage - Module B6 Geographic Representativeness
The use stage related to the operation of the building includes: Land or region, in which the declared product system is
— B6, operational energy use manufactured, used or handled at the end of the product´s
lifespan: Germany
End-of-life stage– Modules C1-C4 and D
The end-of-life stage includes:
Comparability
— C1, de-construction, demolition:
Basically, a comparison or an evaluation of EPD data is only
— C2, transport to waste processing;
possible if all the data sets to be compared were created
— C3, waste processing for reuse, recovery and/or recycling;
according to EN 15804 and the building context, respectively
— C4, disposal;
the product-specific characteristics of performance, are taken
including provision and all transport, provision of all materials,
into account. Background database: GaBi, SP40.
products and related energy and water use.
LCA: Scenarios and additional technical information
Operational energy use (B6) and Operational water use
Characteristic product properties of biogenic carbon
(B7)
Information on describing the biogenic Carbon Content at The use stage is declared for 12 years.
factory gate
Name Value Unit
Name ValueUnit
Energy consumption for 1 year 19,75 kWh
kg
Biogenic carbon content in product 0.01 on mode per day 2 h
C
idle mode per day 22 h
Biogenic carbon content in accompanying kg
0.02 on mode power 5 W
packaging C
idle mode power 2 W
Note: 1 kg of biogenic carbon is equivalent to 44/12 kg of CO .
2 Days per year in use 365 days
End of life (C1-C4)
The following technical scenario information is required for the
C1: The product dismantling from the building is done manually
declared modules.
without environmental burden.
Transport to the building site (A4)
Name Value Unit
Name Value Unit Recycling 0.04 kg
Litres of fuel per 1 kg 0.00276 l/100km Energy recovery 0.04 kg
Transport distance 750 km Landfilling 0.01 kg
Capacity utilisation (including empty runs) 51 % Transportation to Waste Processing Site 50 km
Installation into the building (A5) Region for end of life: Global
Name Value Unit
Reuse, recovery and/or recycling potentials (D), relevant
Waste Packaging (paper) 0,05 kg
scenario information
Collection rate is 100%.
Reference service life
Name Value Unit
Life Span according to the manufacturer 12 a
3 Environmental Product Declaration - dormakaba - Extension module 90 43
LCA: Results
DESCRIPTION OF THE SYSTEM BOUNDARY (X = INCLUDED IN LCA; MND = MODULE OR INDICATOR NOT DECLARED; MNR
= MODULE NOT RELEVANT)
Benefits and
Construction loads beyond
Product stage Use stage End of life stage
process stage the system
boundaries
la ire ta m w a Ry lp p u s tro p s n a rT g n iru tc a fu n a M e h t m o rf tro p s n a rTe tis e h t o t e ta g y lb m e s s A e s U e c n a n e tn ia M ria p e R tn e m e c a lp e R tn e m h s ib ru fe R y g re n e la n o ita re p Oe s u re ta w la n o ita re p Oe s u n o itc u rts n o c -e Dn o itilo m e d tro p s n a rT g n is s e c o rp e ts a W la s o p s iD -e s u e R-y re v o c e R-g n ilc y c e Rla itn e to p
A1 A2 A3 A4 A5 B1 B2 B3 B4 B5 B6 B7 C1 C2 C3 C4 D
X X X X X MND MND MNR MNR MNR X MND X X X X X
RESULTS OF THE LCA - ENVIRONMENTAL IMPACT according to EN 15804+A2: 1 piece Extension module 90 43
Parameter Unit A1-A3 A4 A5 B6 C1 C2 C3 C4 D
GWP-total kg CO 2 eq 3.41E+00 1E-02 7.6E-02 9.59E+01 0 4.64E-04 1.06E-01 1.9E-04 -2.06E-01
GWP-fossil kg CO 2 eq 3.42E+00 9E-03 2E-03 9.54E+01 0 4.43E-04 1.06E-01 1.89E-04 -2.06E-01
GWP-biogenic kg CO 2 eq -1.79E-02 4.23E-04 7.4E-02 3.18E-01 0 2.05E-05 2.47E-06 6.45E-07 1.92E-04
GWP-luluc kg CO 2 eq 5.09E-03 2.18E-07 1.25E-06 1.38E-01 0 1.06E-08 5.98E-06 5.44E-07 -2.81E-04
ODP kg CFC11 eq 4.72E-10 9.66E-19 1.37E-17 2.1E-12 0 4.68E-20 5.34E-17 7E-19 -1.19E-15
AP mol H+ eq 1.91E-02 9.16E-06 2.12E-05 2.11E-01 0 4.44E-07 1.89E-05 1.36E-06 -3E-03
EP-freshwater kg P eq 2.57E-05 1.96E-09 2.67E-09 2.55E-04 0 9.49E-11 8.52E-09 3.24E-10 -1.83E-07
EP-marine kg N eq 3.05E-03 2.92E-06 7.67E-06 4.7E-02 0 1.41E-07 4.25E-06 3.49E-07 -1.98E-04
EP-terrestrial mol N eq 3.64E-02 3.24E-05 9.56E-05 4.92E-01 0 1.57E-06 8.58E-05 3.83E-06 -2E-03
kg NMVOC
POCP 1.01E-02 8.24E-06 2.03E-05 1.28E-01 0 3.99E-07 1.18E-05 1.06E-06 -6.59E-04
eq
ADPE kg Sb eq 7.31E-04 2.75E-10 2.16E-10 2.76E-05 0 1.33E-11 7.32E-10 1.7E-11 -1.15E-04
ADPF MJ 4.14E+01 1.3E-01 2.4E-02 1.68E+03 0 6E-03 4.9E-02 2E-03 -2.8E+00
m3 world eq
WDP 8.53E-01 1.79E-05 9E-03 2.08E+01 0 8.69E-07 1.1E-02 1.98E-05 -7.4E-02
deprived
GWP = Global warming potential; ODP = Depletion potential of the stratospheric ozone layer; AP = Acidification potential of land and water; EP =
Eutrophication potential; POCP = Formation potential of tropospheric ozone photochemical oxidants; ADPE = Abiotic depletion potential for non-fossil
resources; ADPF = Abiotic depletion potential for fossil resources; WDP = Water (user) deprivation potential)
RESULTS OF THE LCA - INDICATORS TO DESCRIBE RESOURCE USE according to EN 15804+A2: 1 piece Extension module
90 43
Parameter Unit A1-A3 A4 A5 B6 C1 C2 C3 C4 D
PERE MJ 1.21E+01 4.09E-04 6.46E-01 7.43E+02 0 1.98E-05 1.62E-01 3.25E-04 -4.41E-01
PERM MJ 7.91E-01 0 -6.42E-01 0 0 0 -1.49E-01 0 0
PERT MJ 1.29E+01 4.09E-04 4E-03 7.43E+02 0 1.98E-05 1.3E-02 3.25E-04 -4.41E-01
PENRE MJ 3.95E+01 1.3E-01 2.4E-02 1.68E+03 0 6E-03 2.01E+00 2E-03 -2.81E+00
PENRM MJ 1.96E+00 0 0 0 0 0 -1.96E+00 0 0
PENRT MJ 4.14E+01 1.3E-01 2.4E-02 1.68E+03 0 6E-03 4.9E-02 2E-03 -2.81E+00
SM kg 0 0 0 0 0 0 0 0 0
RSF MJ 0 0 0 0 0 0 0 0 0
NRSF MJ 0 0 0 0 0 0 0 0 0
FW m3 2.2E-02 7.34E-07 2.21E-04 8.6E-01 0 3.56E-08 2.59E-04 6.25E-07 -1E-03
PERE = Use of renewable primary energy excluding renewable primary energy resources used as raw materials; PERM = Use of renewable primary
energy resources used as raw materials; PERT = Total use of renewable primary energy resources; PENRE = Use of non-renewable primary energy
excluding non-renewable primary energy resources used as raw materials; PENRM = Use of non-renewable primary energy resources used as raw
materials; PENRT = Total use of non-renewable primary energy resources; SM = Use of secondary material; RSF = Use of renewable secondary fuels;
NRSF = Use of non-renewable secondary fuels; FW = Use of net fresh water
RESULTS OF THE LCA – WASTE CATEGORIES AND OUTPUT FLOWS according to EN 15804+A2:
1 piece Extension module 90 43
Parameter Unit A1-A3 A4 A5 B6 C1 C2 C3 C4 D
HWD kg 3.75E-06 1.26E-11 3.53E-11 6.94E-07 0 6.1E-13 1.87E-10 3.78E-11 -8.47E-09
NHWD kg 1.19E-01 1.33E-05 2E-03 1.19E+00 0 6.44E-07 1.1E-02 1.2E-02 -3.2E-02
RWD kg 9.43E-04 1.4E-07 1.26E-06 2.55E-01 0 6.76E-09 1.82E-06 2.82E-08 -9.23E-05
CRU kg 0 0 0 0 0 0 0 0 0
MFR kg 0 0 0 0 0 0 5.2E-02 0 0
MER kg 0 0 0 0 0 0 0 0 0
EEE MJ 1.07E-01 0 1.15E-01 0 0 0 0 0 0
EET MJ 1.95E-01 0 2.08E-01 0 0 0 0 0 0
4 Environmental Product Declaration - dormakaba - Extension module 90 43
HWD = Hazardous waste disposed; NHWD = Non-hazardous waste disposed; RWD = Radioactive waste disposed; CRU = Components for re-use;
MFR = Materials for recycling; MER = Materials for energy recovery; EEE = Exported electrical energy; EET = Exported thermal energy
RESULTS OF THE LCA – additional impact categories according to EN 15804+A2-optional:
1 piece Extension module 90 43
Parameter Unit A1-A3 A4 A5 B6 C1 C2 C3 C4 D
Disease
PM 1.97E-07 4.82E-11 1.18E-10 1.77E-06 0 2.33E-12 2.41E-10 1.68E-11 -2.06E-08
incidence
IR kBq U235 eq 9.1E-02 1.99E-05 1.95E-04 4.18E+01 0 9.65E-07 1.64E-04 2.9E-06 -1.4E-02
ETP-fw CTUe 1.99E+01 9.2E-02 1.1E-02 7.17E+02 0 4E-03 1.8E-02 1E-03 -1.32E+00
HTP-c CTUh 1.2E-09 1.73E-12 6.01E-13 1.98E-08 0 8.38E-14 1.59E-12 2.1E-13 -8.92E-11
HTP-nc CTUh 6.32E-08 7.4E-11 2.61E-11 7.3E-07 0 3.59E-12 1.61E-10 2.31E-11 -7.16E-09
SQP SQP 1.82E+01 3.34E-04 6E-03 5.34E+02 0 1.62E-05 1.5E-02 5.17E-04 -1.22E+00
PM = Potential incidence of disease due to PM emissions; IR = Potential Human exposure efficiency relative to U235; ETP-fw = Potential comparative
Toxic Unit for ecosystems; HTP-c = Potential comparative Toxic Unit for humans (cancerogenic); HTP-nc = Potential comparative Toxic Unit for humans
(not cancerogenic); SQP = Potential soil quality index
Disclaimer 1 – for the indicator IRP
This impact category deals mainly with the eventual impact of low dose ionizing radiation on human health of the nuclear fuel cycle. It
does not consider effects due to possible nuclear accidents, occupational exposure nor due to radioactive waste disposal in
underground facilities. Potential ionizing radiation from the soil, from radon and from some construction materials is also not measured
by this indicator.
Disclaimer 2 – for the indicators ADPE, ADPF, WDP, ETP-fw, HTP-c, HTP-nc, SQP
The results of this environmental impact indicator shall be used with care as the uncertainties on these results are high or as there is
limited experience with the indicator.
References
Standards declarations — Type III environmental declarations —
Principles and procedures.
EN 15804
EN 15804:2019+A2 (in press), Sustainability of construction Radio Equipment Directive (RED)
works — Environmental Product Declarations — Core rules for Directive 2014/53/EU of the European Parliament and of the
the product category of construction products. Council of 16 April 2014 on the harmonisation of the laws of the
Member States relating to the making available on the market
EN 300328 V2.1.1 of radio equipment and repealing Directive 1999/5/EC.
Wideband transmission systems;Data transmission equipment
operating in the 2,4 GHz ISM band and using wide band Registration, Evaluation, Authorisation and Restriction of
modulation techniques; Harmonised Standard covering the Chemicals (REACH)
essential requirements of article 3.2 of Directive 2014/53/EU. Regulation (EC) No 1907/2006 of the European Parliament and
of the Council on the Registration, Evaluation, Authorisation
EN 301489-1 V2.2.0 Draft and Restriction of Chemicals (REACH).
ElectroMagnetic Compatibility (EMC)standard for radio
equipment and services; Part 1: Common technical Restriction of Hazardous Substances (RoHS)
requirements; Harmonised Standard covering the essential Directive on the restriction of the use of certain hazardous
requirements of article 3.1(b) of Directive 2014/53/EU and the substances in electrical and electronic equipment (RoHS),
essential requirements of article 6 of Directive 2014/30/EU. Directive (EU) No 2011/65.
EN 301489-17 V3.2.1 Draft Further References
ElectroMagnetic Compatibility (EMC)standard for radio
equipment and services; Part 17: Specific conditions for IBU 2016
Broadband Data Transmission Systems; Harmonised Standard Institut Bauen und Umwelt e.V.: General Instructions for the
for ElectroMagnetic Compatibility. EPD programme of Institut Bauen und Umwelt e.V. Version 2.0,
Berlin: Institut Bauen und Umwelt e.V., 2021.
EN 50581
EN 50581:2012, Technical documentation for the assessment GaBi ts software
of electrical and electronic products with respect to the Sphera Solutions GmbHGabi Software System and Database
restriction of hazardous substances. for Life Cycle Engineering 1992-2020 Version 10.0.0.71
University of Stuttgart Leinfelden-Echterdingen
EN 62311
EN 62311:2008, Assessment of electronic and electrical GaBi ts documentation
equipment related to human exposure restrictions for GaBi life cycle inventory data documentation (https://www.gabi-
electromagnetic fields. software.com/support/gabi/gabi-database-2020-lci-
documentation/).
EN 62368-1
EN 62368-1:2014, Audio/video, information and communication LCA-tool dormakaba
technology equipment - Part 1: Safety requirements. LCA tool, version 1.0.
Developed by Sphera Solutions GmbH.
ISO 14025
DIN EN ISO 14025:2011-10, Environmental labels and PCR Part A
5 Environmental Product Declaration - dormakaba - Extension module 90 43
PCR – Part A:
Calculation Rules for the Life Cycle As-sessment and PCR Part B
Requirements on the Project Re-port according to EN PCR – Part B: Requirements on the EPD for Building Hardware
15804+A2:2019, Version 1.0, Institut Bauen und Umwelt e.V., product, version 1.3, Institut Bauen und Umwelt e.V., www.ibu-
www.ibu-epd.com. epd.com, 2019.
6 Environmental Product Declaration - dormakaba - Extension module 90 43
Publisher
Institut Bauen und Umwelt e.V. +49 (0)30 3087748- 0
Hegelplatz 1 info@ibu-epd.com
10117 Berlin www.ibu-epd.com
Germany
Programme holder
Institut Bauen und Umwelt e.V. +49 (0)30 3087748- 0
Hegelplatz 1 info@ibu-epd.com
10117 Berlin www.ibu-epd.com
Germany
Author of the Life Cycle Assessment
Sphera Solutions GmbH +49 711 341817-0
Hauptstraße 111- 113 info@sphera.com
70771 Leinfelden-Echterdingen www.sphera.com
Germany
Owner of the Declaration
dormakaba International Holding GmbH +49 2333 793-0
DORMA Platz 1 info.de@dormakaba.com
58256 Ennepetal www.dormakaba.com
Germany
7 Environmental Product Declaration - dormakaba - Extension module 90 43
