ENVIRONMENTAL PRODUCT DECLARATION
as per ISO 14025 and EN 15804+A2
Owner of the Declaration Knauf Ceiling Solutions GmbH & Co. KG
Publisher Institut Bauen und Umwelt e.V. (IBU)
Programme holder Institut Bauen und Umwelt e.V. (IBU)
Declaration number EPD-KNA-20240458-IBA1-EN
Issue date 06.12.2024
Valid to 05.12.2029
Heradesign Fine A2 25 mm
Knauf Ceiling Solutions GmbH & Co. KG
www.ibu-epd.com | https://epd-online.com
1. General Information
Knauf Ceiling Solutions GmbH & Co. KG Heradesign Fine A2 25 mm
Programme holder Owner of the declaration
IBU – Institut Bauen und Umwelt e.V. Knauf Ceiling Solutions GmbH & Co. KG
Hegelplatz 1 Elsenthal 15
10117 Berlin 94481 Grafenau
Germany Germany
Declaration number Declared product / declared unit
EPD-KNA-20240458-IBA1-EN 1 m² Heradesign Fine A2 25 mm (Euroclass A2).
This declaration is based on the product category rules: Scope:
Wood cement - Mineral-bonded wooden composites, 01.08.2021 This document refers to 1 m² of Heradesign Fine A2 25 mm (Euroclass A2)
(PCR checked and approved by the SVR) with a surface weight of 19 kg/m² manufactured at the production facility in
Ferndorf (Austria). The product is a magnesite bonded wood wool panel.
Issue date The owner of the declaration shall be liable for the underlying information
and evidence; the IBU shall not be liable with respect to manufacturer
06.12.2024
information, life cycle assessment data and evidences.
The EPD was created according to the specifications of EN 15804+A2. In
Valid to
the following, the standard will be simplified as EN 15804.
05.12.2029
Verification
The standard EN 15804 serves as the core PCR
Independent verification of the declaration and data according to ISO
14025:2011
internally X externally
Dipl.-Ing. Hans Peters
(Chairman of Institut Bauen und Umwelt e.V.)
Florian Pronold Matthias Schulz,
(Managing Director Institut Bauen und Umwelt e.V.) (Independent verifier)
1 Environmental Product Declaration - Knauf Ceiling Solutions GmbH & Co. KG - Heradesign Fine A2 25 mm
2. Product
The products are delivered packed in cardboard on pallets.
2.1 Product description/Product definition
Heradesign panels are wood wool panels in accordance with 2.5 Base materials/Ancillary materials
EN 13168 and/or EN 13964, manufactured from wood wool and
Composition of Heradesign products:
mineral binding agents.
Name Value Unit
Product names: 17 (+/-
Spruce (Picea abies) %
1,7)
Heradesign Fine A2 25 mm Anorganic binder 37 (+/- 3) %
For the marketing of the products in the European 4 (+/-
Magnesium sulphate (MgSO4) CAS: 7487-88-9 %
Union/European Free Trade Association (EU/EFTA) (with the 0,4)
exception of Switzerland) Regulation (EU) No. 305/2011 (CPR)
Water (H2O) CAS: 7732-16-5 (solvent for
applies. 10 (+/- 3) %
Magnesiumsulphate)
The products require a declaration of performance taking into
Dolomite (CaMg(CO3)2 ) CAS: 16389-88-1 32 (+/- 3) %
account EN 13168:2012+A1:2015, Thermal insulation products
for buildings - Factory made wood wool (WW) products - The spruce wood is procured from sustainable forest
Specification or EN 13964:2014, Suspended ceilings - management and serves as a substrate. Caustic magnesia is
Requirements and test methods and the CE marking. extracted from regional magnesite raw material. Magnesium
sulphate serves as a co-binding partner; water is partially
The respective national regulations apply to their use. bound in the form of crystal water and partially contained as
residual moisture. No biocides or fire retardants are used in the
2.2 Application
product.
Heradesign acoustic panels are primarily used as For optical reasons, the finished products are dyed on the
acoustic/decorative wall and ceiling panelling in offices, visible side using dispersion paint.
kindergartens etc.
At least one sub-product contains substances of the candidate
2.3 Technical Data
list (date 27.06.2024) above 0.1 % by mass: no.
Product-specific values can be found at
www.knaufceilingsolutions.com
The product contains other cancerogenic, mutagenic,
Constructional data reprotoxic (CMR) substances of category 1A or 1B that are not
on the candidate list, above 0,1 % by mass in at least one part
Name Value Unit
product: no.
Gross density acc. to EN 1602 760 kg/m3
Grammage 19,0 kg/m2 Biocidal products have been added to this construction product
Thickness 25 mm or it has been treated with biocidal products (it is therefore a
Bending strength (longitudinal) n.r. N/mm2 treated product within the meaning of the Biocidal Products
Regulation (EU) No 528/2012): no.
Bending strength (transverse) n.r. N/mm2
E-module (longitudinal) n.r. N/mm2 No fire retardants were used in the product.
E-module (transverse) n.r. N/mm2
2.6 Manufacture
Tensile strength rectangular n.r. N/mm2
Thermal conductivity acc. to EN 12667 0.11 W/(mK) 2.6.1 Raw material
Water vapour diffusion resistance factor acc. Spruce wood is stored as trunks 2 metres in length. Depending
2 - 5 -
to DIN 4108-4 on climate conditions, storage lasts around 6-12 months. The
Moisture content at 23 °C, 80% 11 M.-% trunks are transported by conveyor belts to a multi-rip saw, cut
into pieces and processed as wood wool using a planing
Coefficient of thermal expansion n.r. 10-6K-1
machine. The binding agent components are stored in steel
Swelling (air-dry to water-saturated) n.r. % silos.
Sound absorption coefficient (only with up to
%
reference to component design) 0,95 2.6.2 Mixer
Wood wool, as well as a binding agent and a magnesium
n.r. = not relevant
sulphate solution, are required for generating a mixture for
wood wool pellets. These components are transported to a
Performance data of the product in accordance with the
mixer where they are processed to form the requisite formula.
declaration of performance with respect to its essential
characteristics to EN 13168:2012+A1:2015, Thermal insulation
2.6.3 Scattering and shaping
products for buildings - Factory made wood wool (WW)
The mixture is scattered onto a steel band and passed through
products - Specification or rather EN 13964:2014, Suspended
a binding channel, whereby it is separated from the room by a
ceilings - Requirements and test methods.
second horizontal steel strip as well as two side strips. An
2.4 Delivery status endless product is produced on leaving the twin belt. The raw
Wood wool products are exclusively available as panels. goods are then cut to the desired length.
Typical dimensions:
Lengths: 1250 mm, 1200 mm and on request
Widths: 625 mm, 600 mm
Thicknesses: 25 mm
2 Environmental Product Declaration - Knauf Ceiling Solutions GmbH & Co. KG - Heradesign Fine A2 25 mm
and disposed of where such waste incurs.
2.10 Condition of use
No emissions are to be expected during the use phase of the
Heradesign acoustic panels because the ingredients are firmly
bound in the state of use.
Heradesign acoustic panels do not require any maintenance
from which significant effects on the environment can be
expected.
Cleaning is done by sweeping off occasionally. No effects are
assumed in Module B3 -Repair- because the repair of
2.6.4 Interim storage and picking Heradesign acoustic panels is rarely necessary. In the case of a
The products are put into interim storage for 3-5 days (drying repair, the entire board is replaced, which would correspond to
and maturing process). The requisite edge design is then the environmental impact declared in modules A1–A3.
produced on so-called double-end profiling machines. No effects are assumed for modules B4 and B5 either, because
Edge processing: 18 standard edges are possible. with Heradesign acoustic panels, when used as intended, no
replacement or renewal is required during the service life of 50
years. Modules B6 (energy use for operating the building) and
B7 (water use for operating the building) are not relevant for
Heradesign acoustic panels.
2.11 Environment and health during use
According to current knowledge, hazards to water, air and soil
cannot arise if the described products are used as intended.
Heradesign products meet the requirements of the Blue Angel
(RAL UZ 132, low-emission thermal insulation materials and
2.6.5 Dyeing, packaging and shipping suspended ceilings for use in buildings, October 2010). Test
The requisite colour is applied in a dyeing plant, followed by reports from eurofins confirm the fulfilment of the requirements
packaging and storage. for building structures with regard to health protection (ABG),
Dyeing: Possible in many RAL colours (left) draft 31.08.2017, as well as the achievement of class A+ of the
Products ready for storage (right) French Volatile Organic Compound (VOC) regulation
(regulation March and April 2011 ( DEVL1101903D and
DECL1104875A).
2.12 Reference service life
The service life of Heradesign products is 50 years, but it
depends mainly on the life of the building. Due to the mineral
binder, no ageing processes are known.
2.13 Extraordinary effects
Fire
Reaction to fire: Class A2-,s1-, d0 according EN 13501-1
2.7 Environment and health during manufacturing
The site in Ferndorf has introduced a safety management Reaction to fire
system in accordance with BS OHSAS 18001, whereby Bureau Name Value
Veritas confirms compliance with the specified requirements in Building material class acc. to EN 13501-1 A2
the form of a corresponding certificate.
Burning droplets acc. to EN 13501-1 d0
In order to safeguard all environmental protection measures
Smoke gas development acc. to EN 13501-1 s1
and drive energy efficiency measures during the manufacturing
process, the site has opted for ISO 14001 as well as ISO 50001
certification. The Bureau Veritas certificate confirms compliance Water
with the specified requirements. The manufacturing plant has a Heradesign acoustic panels are intended for indoor use. Should
"zero waste policy", all production-related waste (cutting waste, an unforeseen water effect, e.g. a flood, occur, the panels are
production residues) is returned to the production process in fully functional again after drying. There is no impairment of the
the course of raw material preparation. environment to be expected.
This also applies to washing water, which is also 100 %
recycled in the production process. Mechanical destruction
This point is not relevant for a wood-wool building board, as
2.8 Product processing/Installation
there is no environmental impact in case of unforeseen
The type of mounting is described in detail in the brochure destruction. It would be more an optical defect.
"System solutions". In it, the possible systems, concealed
systems, screw systems etc. are dealt with in detail. 2.14 Re-use phase
Uncontaminated Heradesign panels can be reused. The
For further information, in addition to the "System Solutions" following reuse options are available:
brochure, individual processing videos can also be downloaded
from the website www.knaufceilingsolutions.com Re-use:
Clean Heradesign panels can be re-used.
2.9 Packaging
By screw mounting or an inserted T-rail, re- and new mounting
Heradesign acoustic panels are supplied in protective is easily possible without damaging the product.
cardboard packaging on untreated wooden pallets.
It must be ensured that the packaging materials are separated
3 Environmental Product Declaration - Knauf Ceiling Solutions GmbH & Co. KG - Heradesign Fine A2 25 mm
Composting: Waste code EAK-code: 17 01 07
Wood wool panels, mechanically shredded, can be converted
into compost material by enrichment with appropriate bacteria. Thermal recycling
This material can then be used for soil improvement in In the manufacturing plant, waste plates can be recycled to
agriculture. binder in a rotary kiln process. This would be the preferred way
in terms of a functioning recycling economy.
2.15 Disposal
If the above-mentioned recycling options are not practicable, 2.16 Further information
the slab residues arising on the construction site as well as Further information, for example, product data sheets, safety
slabs from demolition activities can easily be disposed of in data sheets or declarations of performances are available on
landfills without pretreatment due to their predominantly mineral the website: www.knaufceilingsolutions.com
content.
3. LCA: Calculation rules
Module C3 | Waste processing
3.1 Declared Unit The declared scenario assumes landfilling of the product.
This EPD refers to a declared unit of 1 m² of Heradesign Fine Referring environmental impacts are accounted for in module
A2 25 mm (Euroclass A2). The declared unit refers to a surface C4. Therefore, no environmental impacts from waste
weight of 19 kg/m². processing of the product are expected in C3.
Declared unit
Module C4 | Disposal
Name Value Unit
Modul C4 declares the environmental impacts from landfilling
Declared unit 1 m2 after use of the product. The biogenic carbon in the wood share
Grammage 19 kg/m2 of the product is treated as emissions of biogenic CO from the
2
Grammage 0.019 t/m² technosphere to the natural environment.
Conversion factor to 1 t 52.63 m²/t
Module D | Benefits and loads beyond the system
Layer thickness 0.025 m
boundary
Other declared units are allowed if the conversion is shown The declared scenario assumes landfilling of the product.
transparently. Referring environmental impacts are accounted for in module
C4. No benefits or loads outside the system boundary in
Various Heradesign products are manufactured at the site. The Module D are to be expected.
allocation of product specific material and energy flows for the
different Euroclasses (B and A2) produced is based on the 3.3 Estimates and assumptions
composition of the referring products. All assumptions are verified through detailed documentation
and correspond to the best possible representation of reality
3.2 System boundary
based on the available data. Regional applicability of the used
The life cycle assessment of Heradesign acoustic panels background data refers to average data under European or
includes a cradle-to-gate analysis of the environmental impacts German conditions taken from the GaBi database. German
with modules C1–C4 and module D (A1–A3, + C + D). data were used for the Austrian market whenever European or
Subsequent life cycle phases are part of the analysis: regionalised average data were not available.
Module A1–A3 | Production stage 3.4 Cut-off criteria
The production stage includes upstream burdens of raw All inputs and outputs for which data are available and a
materials (wood, binding agents, recalcination, auxiliaries, etc.) significant impact is expected are included in the LCA model.
and the corresponding transports to the production site in Data gaps are filled with conservative assumptions from
Ferndorf (Austria). Material and energy flows needed for the average data (when available) or with generic data and are
mixing of the components, scattering and shaping, interim documented accordingly. Only data with a contribution of less
storage and picking as well as dyeing and packaging were than 1 % were cut off. Ignoring such data is justified based on
specifically recorded. In addition, the recalcination process for the insignificance of the expected effect. Processes, materials
the provision of Knauf Sekundärkauster is considered. The or emissions known to have a significant contribution to the
representation of all specific input and output flows is thus environmental effects of the products under examination have
based on company-specific foreground data. 100 % green not been neglected. The data collection was verified using
electricity is used in the production. Thermal energy results available comparative values. It is assumed that the data have
from energy recovery from the recalcination process been completely recorded and that the overall total of ignored
supplemented by natural gas. input flows does not amount to more than 5 % of the total
energy and mass flows. Environmental impacts of machines,
Module C1 | Deconstruction and demolition plant and infrastructure were not included.
Disassembly of the product is done either manually or using
smaller tools. Referring energy demand is considered to be 3.5 Background data
negligible. This study uses generic background data for the evaluation of
upstream environmental impacts from GaBi databases (GaBi
Module C2 | Transport to disposal 10; 2022.2).
The transport to the disposal of the material is estimated
3.6 Data quality
declaring a 50 km radius to the landfill. In reality, this scenario
may vary depending on the actual location of deconstruction Data collection is based on product-specific questionnaires. It
and referring waste treatment. follows an iterative process clarifying questions via e-mail,
telephone calls or in personal meetings. Intensive discussions
between Knauf Ceiling Solutions and Daxner & Merl results in
4 Environmental Product Declaration - Knauf Ceiling Solutions GmbH & Co. KG - Heradesign Fine A2 25 mm
an accurate mapping of product-related material and energy
flows. This leads to a high quality of foreground data collected. 3.9 Allocation
Data collection relies on a consistent process according to ISO The life cycle assessment considers the material inherent
14044. properties of wood (carbon content and primary energy
content) and relies on its physical relations.
The technological, geographical and time-related
representativeness of the database was kept in mind when The annually used raw material and referring energy flows at
selecting background data. Whenever specific data were Ferndorf were allocated to the specific products based on the
missing, either generic datasets or representative average data square meters produced yearly.
were used instead. The implemented GaBi background
datasets refer to the latest versions available (not more than Wooden residues result from the production process. As they
ten years old) and are carefully chosen. account for less than 1 % of the yearly turnover of the
organisation, they were not considered as co-products.
3.7 Period under review Referring quantities were cut-off.
Foreground data were collected in the 2018 production year,
and the data are based on the volumes produced on an annual 3.10 Comparability
basis. Basically, a comparison or an evaluation of EPD data is only
possible if all the data sets to be compared were created
3.8 Geographic Representativeness according to EN 15804 and the building context, respectively
Land or region, in which the declared product system is the product-specific characteristics of performance, are taken
manufactured, used or handled at the end of the product´s into account. The GaBi background database was used to
lifespan: Austria calculate the LCA (GaBi 10; 2022.2).
4. LCA: Scenarios and additional technical information
Installation (A5)
Characteristic product properties of biogenic carbon
The End of Life of product packaging is not declared in module
The biogenic carbon content quantifies the amount of biogenic
A5.
carbon in the declared building product.
Name Value Unit
Production stage (A1–A3) Packaging (cardboard) 0.083 kg
In module A1-A3 the absorption of 3.65 kg biogenic CO 2 per Packaging (pallets) 0.22 kg
declared unit in the Heradesign acoustic panels has been
The biogenic carbon content of the cardboard and the wooden
considered, due to the carbon stored in the wood.
pallets has been treated CO -neutral and not accounted for as
2
In the recalcination process, the emissions of 0.47 kg of carbon storage.
biogenic CO were balanced in module A1-A3.
2
Information for describing the biogenic carbon content at
End of Life (C1–C4)
factory gate
Name Value Unit
Name ValueUnit
Landfilling 19 kg
kg
Biogenic carbon content in product 1
C During landfilling 3.65 kg of biogenic CO remain in the
2
Biogenic carbon content in accompanying kg product. Due to the binding properties of magnesite,
0.14
packaging C Heradesign acoustic panels can be deposited. This
corresponds to a representative scenario. Long-term landfill gas
Note: 1 kg biogenic Carbon is equivalent to 44/12 kg of CO
2 measurements as well as periodic material withdrawals from
the deposited products confirm the retention of the biogenic
bound carbon during landfilling.
In accordance with the requirements of EN 15804+A2, the
biogenic carbon in the wood of the products is declared as
emissions of biogenic CO from the technosphere into the
2
natural environment in module C4.
5 Environmental Product Declaration - Knauf Ceiling Solutions GmbH & Co. KG - Heradesign Fine A2 25 mm
5. LCA: Results
The following table contains the LCA results for a declared unit of 1 m² Heradesign Fine A2 25 mm (Euroclass A2) with a surface
weight of 19 kg/m². This corresponds to 0.019 t/m².
DESCRIPTION OF THE SYSTEM BOUNDARY (X = INCLUDED IN LCA; MND = MODULE OR INDICATOR NOT DECLARED; MNR
= MODULE NOT RELEVANT)
Benefits and
Construction loads beyond
Product stage Use stage End of life stage
process stage the system
boundaries
la ire ta m w a Ry lp p u s tro p s n a rT g n iru tc a fu n a M e h t m o rf tro p s n a rTe tis e h t o t e ta g y lb m e s s A e s U e c n a n e tn ia M ria p e R tn e m e c a lp e R tn e m h s ib ru fe R y g re n e la n o ita re p Oe s u re ta w la n o ita re p Oe s u n o itc u rts n o c -e Dn o itilo m e d tro p s n a rT g n is s e c o rp e ts a W la s o p s iD -e s u e R-y re v o c e R-g n ilc y c e Rla itn e to p
A1 A2 A3 A4 A5 B1 B2 B3 B4 B5 B6 B7 C1 C2 C3 C4 D
X X X MND MND MND MND MNR MNR MNR MND MND X X X X X
RESULTS OF THE LCA - ENVIRONMENTAL IMPACT according to EN 15804+A2: 1 m² Heradesign Fine A2 25 mm (19 kg/m²),
Euroclass A2
Parameter Unit A1-A3 C1 C2 C3 C4 D
Global Warming Potential total (GWP-total) kg CO 2 eq 3.66E+00 0 5.76E-02 0 3.92E+00 0
Global Warming Potential fossil fuels (GWP-fossil) kg CO 2 eq 7.37E+00 0 5.72E-02 0 2.84E-01 0
Global Warming Potential biogenic (GWP-biogenic) kg CO 2 eq -3.71E+00 0 0 0 3.64E+00 0
Global Warming Potential luluc (GWP-luluc) kg CO 2 eq 1.78E-03 0 3.84E-04 0 5.23E-04 0
Depletion potential of the stratospheric ozone layer (ODP) kg CFC11 eq 9.45E-12 0 5.6E-15 0 6.66E-13 0
Acidification potential of land and water (AP) mol H+ eq 1.41E-02 0 1.91E-04 0 2.01E-03 0
Eutrophication potential aquatic freshwater (EP-freshwater) kg P eq 1.38E-05 0 2.04E-07 0 4.81E-07 0
Eutrophication potential aquatic marine (EP-marine) kg N eq 4.48E-03 0 8.71E-05 0 5.14E-04 0
Eutrophication potential terrestrial (EP-terrestrial) mol N eq 4.83E-02 0 9.76E-04 0 5.65E-03 0
Formation potential of tropospheric ozone photochemical oxidants kg NMVOC
1.26E-02 0 1.71E-04 0 1.56E-03 0
(POCP) eq
Abiotic depletion potential for non fossil resources (ADPE) kg Sb eq 6.15E-07 0 5.75E-09 0 2.91E-08 0
Abiotic depletion potential for fossil resources (ADPF) MJ 7.83E+01 0 7.49E-01 0 3.71E+00 0
m3 world eq
Water use (WDP) 2.97E-01 0 6.38E-04 0 3.11E-02 0
deprived
RESULTS OF THE LCA - INDICATORS TO DESCRIBE RESOURCE USE according to EN 15804+A2: 1 m² Heradesign Fine A2 25
mm (19 kg/m²), Euroclass A2
Parameter Unit A1-A3 C1 C2 C3 C4 D
Renewable primary energy as energy carrier (PERE) MJ 1.96E+01 0 5.19E-02 0 5.57E-01 0
Renewable primary energy resources as material utilization
MJ 3.78E+01 0 0 0 0 0
(PERM)
Total use of renewable primary energy resources (PERT) MJ 5.74E+01 0 5.19E-02 0 5.57E-01 0
Non renewable primary energy as energy carrier (PENRE) MJ 7.83E+01 0 7.52E-01 0 3.72E+00 0
Non renewable primary energy as material utilization (PENRM) MJ 0 0 0 0 0 0
Total use of non renewable primary energy resources (PENRT) MJ 7.83E+01 0 7.52E-01 0 3.72E+00 0
Use of secondary material (SM) kg 1.43E+00 0 0 0 0 0
Use of renewable secondary fuels (RSF) MJ 0 0 0 0 0 0
Use of non renewable secondary fuels (NRSF) MJ 0 0 0 0 0 0
Use of net fresh water (FW) m3 2.49E-02 0 5.99E-05 0 9.43E-04 0
RESULTS OF THE LCA – WASTE CATEGORIES AND OUTPUT FLOWS according to EN 15804+A2:
1 m² Heradesign Fine A2 25 mm (19 kg/m²), Euroclass A2
Parameter Unit A1-A3 C1 C2 C3 C4 D
Hazardous waste disposed (HWD) kg 4.99E-08 0 3.98E-12 0 1.91E-10 0
Non hazardous waste disposed (NHWD) kg 6.26E-01 0 1.22E-04 0 1.9E+01 0
Radioactive waste disposed (RWD) kg 1.16E-03 0 1.4E-06 0 4.13E-05 0
Components for re-use (CRU) kg 0 0 0 0 0 0
Materials for recycling (MFR) kg 0 0 0 0 0 0
Materials for energy recovery (MER) kg 0 0 0 0 0 0
Exported electrical energy (EEE) MJ 0 0 0 0 0 0
Exported thermal energy (EET) MJ 0 0 0 0 0 0
RESULTS OF THE LCA – additional impact categories according to EN 15804+A2-optional:
1 m² Heradesign Fine A2 25 mm (19 kg/m²), Euroclass A2
Parameter Unit A1-A3 C1 C2 C3 C4 D
6 Environmental Product Declaration - Knauf Ceiling Solutions GmbH & Co. KG - Heradesign Fine A2 25 mm
Disease
Incidence of disease due to PM emissions (PM) ND ND ND ND ND ND
incidence
Human exposure efficiency relative to U235 (IR) kBq U235 eq ND ND ND ND ND ND
Comparative toxic unit for ecosystems (ETP-fw) CTUe ND ND ND ND ND ND
Comparative toxic unit for humans (carcinogenic) (HTP-c) CTUh ND ND ND ND ND ND
Comparative toxic unit for humans (noncarcinogenic) (HTP-nc) CTUh ND ND ND ND ND ND
Soil quality index (SQP) SQP ND ND ND ND ND ND
The additional and optional impact categories according to EN 15804+A2 are not declared, as the uncertainty of these indicators is to
be classified as high.
Disclaimer – for the indicators 'abiotic depletion potential for non-fossil resources', 'abiotic depletion potential for fossil resources',
'water (user) deprivation potential, deprivation-weighted water consumption':
The results of this environmental impact indicator shall be used with care as the uncertainties on these results are high as there is
limited experience with the indicator.
6. LCA: Interpretation
The following interpretation contains a summary of the LCA A2 25 mm (Euroclass A2).
results referenced to a declared unit of 1 m² Heradesign Fine
A comparison of the individual life-cycle phases results in a What's more, energy provision for the production at
clear dominance of the production phase (modules A1-A3). Ferndorf represents another important factor in the
The environmental effects in the production phase are mainly environmental profile of Heradesign acoustic panels.
dominated by the upstream production of caustic calcined
magnesium oxide in the supply chain of Knauf Ceiling The amount of wood stored in the product refers to a negative
Solutions. Direct emissions from the calcination process as well contribution to global warming potential. This is due to the
as energy provision for the process account for the major sequestration of biogenic carbon of wood during tree growth.
environmental impacts in this context. The chosen background The sequestered carbon does not contribute to global warming
data refers to a realistic representation of the upstream as long as it is stored in the biomass. In the case of landfilling,
processes as far as possible. this carbon content is stored in the product. If the material is
used as secondary material after deconstruction, the stored
carbon is emitted during recalcination.
7 Environmental Product Declaration - Knauf Ceiling Solutions GmbH & Co. KG - Heradesign Fine A2 25 mm
7. Requisite evidence
Heradesign acoustic panels are certified with the German Result: According to the test report, the product fulfils the
ecolabel "Blue Angel" (RAL-UZ 132) as well as the Danish requirements of the French VOC-Ordinance, the AgBB
product quality seal for indoor climate (certificate Nr. 056) as (Committee for health-related evaluation of building products)
certificate for the environmental friendliness of the products. schema, the Belgian regulations, the Indoor Air Comfort Gold
Standard, the BLUE ANGEL, BREEAM NOR and LEED v4.
7.1 Testing pretreatment of substances used
No waste wood is used for the production of Heradesign AgBB result overview (28 days)
acoustic panels.
7.2 Leaching
Not applicable. Heradesign products are designed for indoor
use, a leaching measurement is not useful.
7.3 VOC emissions
Testing authority: Eurofins Product Testing A/S
Test report: VOC Emissionsprüfbericht Indoor Air Comfort
GOLD (31.08.2021)
Number: 392-2021-00351002_A_EN
Test period: 28.07.-25.08.2021
8. References
Standards declarations - Type III environmental declarations - Principles
and procedures.
DIN 4108-4
DIN 4108-4:2017-03, Thermal insulation and energy economy ISO 14044
in buildings - Part 4: Hygrothermal design values. ISO 14044:2006-07, Environmental management - Life cycle
assessment - Requirements and guidelines.
EN 1602
DIN EN 1602:2013-05, Thermal insulating products for building ISO 50001
applications - Determination of the apparent density. EN ISO 50001:2018, Energy management systems -
Requirements with guidance for use.
EN 12667
DIN EN 12667:2001-05, Thermal performance of building BS OHSAS 18001
materials and products - Determination of thermal resistance by BS OHSAS 18001:2007, Occupational Health and Safety
means of guarded hot plate and heat flow meter methods - Assessment Series.
Products of high and medium thermal resistance.
EN 13168 Further literature
EN 13168:2012+A1:2015, Thermal insulation products for
buildings - Factory made wood wool (WW) products – AgBB
Specification. Ausschuss zur gesundheitlichen Bewertung von Bauprodukte
(AgBB) (Committee for health-related evaluation of building
EN 13501 products): Vorgehensweise bei der gesundheitlichen
EN 13501-1:2007+A1:2009, Fire classification of construction Bewertung der Emissionen von flüchtigen organischen
products and building elements. Verbindungen (VOC und SVOC) aus Bauprodukten.
EN 13964 EAK-code
EN 13964:2014-04-15, Suspended ceilings - Requirements and EAK-code 17 01 07: European Waste Catalogue: Mixtures of
test methods. concrete, brick, tiles and ceramics with the exception of 17 01
06.
EN 15804
DIN EN 15804:2012+A2 2019+AC:2021, Sustainability of ECHA Candidate List
construction works - Environmental Product Declarations - Core Candidate List of substances of very high concern for
rules for the product category of construction products. Authorisation (ECHA Candidate List), retrieved June 27.2024,
published in accordance with Article 59(10) of the REACH
ISO 9001 Regulation. Helsinki: European Chemicals Agency.
EN ISO 9001:2015, Quality management systems -
Requirements. GaBi
GaBi 10, Software-System and Database for Life Cycle
ISO 14001 Engineering. DB 2022.2. Sphera, 1992–2022. Available at:
EN ISO 14001:2015, Environmental management systems - http://documentation.gabisoftware.com
Requirements with guidance for use.
IBU 2021
ISO 14025 Institut Bauen und Umwelt e.V.: General Programme
DIN EN ISO 14025:2011-10, Environmental labels and Instructions for the Preparation of EPDs at the Institut Bauen
8 Environmental Product Declaration - Knauf Ceiling Solutions GmbH & Co. KG - Heradesign Fine A2 25 mm
und Umwelt e.V. (IBU). Version 2.0, Berlin: Institut Bauen und PCR: Wood cement - Mineral-bonded wooden composites
Umwelt e.V., 2021. www.ibuepd.com Product category rules for building-related products and
services. Teil B: Requirements on the EPD for Wood cement -
PCR part A Mineral-bonded wooden composites, Version v10. Berlin:
Product category rules for building-related products and Institut Bauen und Umwelt e.V. (Hrsg.), 2024.
services. Part A: Calculation rules for the life cycle assessment
and requirements on the project report according to
EN15804+A2:2019. Version 1.3, Berlin: Institut Bauen und
Umwelt e.V. (Hrsg.), 2022.
9 Environmental Product Declaration - Knauf Ceiling Solutions GmbH & Co. KG - Heradesign Fine A2 25 mm
Publisher
Institut Bauen und Umwelt e.V. +49 (0)30 3087748- 0
Hegelplatz 1 info@ibu-epd.com
10117 Berlin www.ibu-epd.com
Germany
Programme holder
Institut Bauen und Umwelt e.V. +49 (0)30 3087748- 0
Hegelplatz 1 info@ibu-epd.com
10117 Berlin www.ibu-epd.com
Germany
Author of the Life Cycle Assessment
Daxner & Merl GmbH +43 676 849477826
Schleifmühlgasse 13/24 office@daxner-merl.com
1040 Wien www.daxner-merl.com
Austria
Owner of the Declaration
Knauf Ceiling Solutions GmbH & Co. KG 0049 8552 422 0
Elsenthal 15 ceiling.solutions@knauf.com
94481 Grafenau www.knaufceilingsolutions.com
Germany
10 Environmental Product Declaration - Knauf Ceiling Solutions GmbH & Co. KG - Heradesign Fine A2 25 mm
