ENVIRONMENTAL PRODUCT DECLARATION
as per ISO 14025 and EN 15804+A1
Owner of the Declaration Etex Building Performance International
Programme holder Institut Bauen und Umwelt e.V. (IBU)
Publisher Institut Bauen und Umwelt e.V. (IBU)
Declaration number EPD-PMT-20210296-IBC1-EN
Issue date 23.11.2021
Valid to 22.11.2026
PROMATECT®-100
Mineral bound light weight fire protective boards
Promat
www.ibu-epd.com | https://epd-online.com
Umwelt Produktdeklaration Name des Herstellers – Name des Produkts
1. General Information
Etex Building Performance NV PROMATECT®-100
Programme holder Owner of the declaration
IBU – Institut Bauen und Umwelt e.V. Etex Building Performance International
Panoramastr. 1 500 Rue Marcel Demonque
10178 Berlin F-84915 Avignon
Germany France
Declaration number Declared product / declared unit
EPD-PMT-20210296-IBC1-EN The functional unit is 1 m² of PROMATECT®-100 with
a thickness of 15 mm.
This declaration is based on the product Scope:
category rules: The life cycle assessment is based on production data
Calcium silicate insulating materials, 11.2017 of PROMATECT®-100 of the year 2019 at the
(PCR checked and approved by the SVR) production site Tisselt, Belgium.
Issue date
23.11.2021 The owner of the declaration shall be liable for the
underlying information and evidence; the IBU shall not
Valid to be liable with respect to manufacturer information, life
cycle assessment data and evidences.
22.11.2026
The EPD was created according to the specifications
of EN 15804+A1. In the following, the standard will be
simplified as EN 15804.
Verification
The standard EN 15804 serves as the core PCR
Independent verification of the declaration and data
according to ISO 14025:2010
Dipl. Ing. Hans Peters internally x externally
(chairman of Institut Bauen und Umwelt e.V.)
Dr. Alexander Röder Vito D'Incognito
(Managing Director Institut Bauen und Umwelt e.V.)) (Independent verifier)
2. Product
2.1 Product description/Product definition
Constructional data
PROMATECT®-100 are fire protective calcium silicate Name Value Unit
boards, mineral bound with mineral fillers. Gross density 23°C, 50% RH;
800 - 970 kg/m3
according to ETA 06/0219
For the placing of the product on the market in the Compressive strength according
6.6 N/mm2
European Union/European Free Trade Association to EN 826
EU/EFTA (with the exception of Switzerland) the Tensile strength (perpendicular)
0.043 N/mm2
Regulation (EU) No. 305/2011 (CPR) applies. The according to EN 1607
products need a declaration of performance taking into Flexural strength according to EN
>5 N/mm2
consideration ETA 06/0219_2018-06- 12467
25_PROMATECT®-100 and the CE-marking. For the Thermal conductivity according to
0.27 W/(mK)
application and use the respective national provisions EN 12667
apply. Water vapour diffusion resistance
3 -
factor according to EN 12572
2.2 Application Tensile strength (parallel)
1.21 N/mm^2
according to EN 1608
PROMATECT®-100 boards are used in interior
Values are guidance values and do not reflect a
building applications where normal to high levels of fire
statistical evaluation or guaranteed value.
resistance are required.
Performance data of the product in accordance with
the declaration of performance with respect to its
2.3 Technical Data
essential characteristics according to ETA 06/0219.
2 Environmental Product Declaration Etex Building Performance NV – PROMATECT®-100
2.8 Product processing/Installation
2.4 Delivery status The fire protective board is cut and machined using
PROMATECT®-100 fire protective calcium silicate conventional woodworking equipment.
boards are available in 1200 x 2500 mm and in Fixing the boards will require appropriate means,
thicknesses 8,10,12,15,18,20 and 25 mm. which will depend upon the application and bearing
structure. Boards can be installed using screws or
glues.
2.5 Base materials/Ancillary materials Industrial and environmental protection are assured
Main raw materials used (in weight percentages): through training and coaching staff on safety and
- sand: 5-20 % environmental impacts. Dust levels are kept low by
- lime: 2-15 % performing dust extraction. Noise is reduced by noise
- calcium silicate: 2-15 % insulation on the machines and ear protection is
- gypsum: >50 % provided for persons entering the production area.
- fibres: <3 % Regular measurements on noise and dust are
Reaction is performed in an aqueous suspension. performed and show conformity to the permitted
levels.
This article contains substances listed in the candidate All national, local and other applicable safety
list (date: 19.01.2021) exceeding 0.1 percentage by regulations are complied with.
mass: no.
This article contains other carcinogenic, mutagenic, 2.9 Packaging
reprotoxic (CMR) substances in categories 1A or 1B All fire protection boards are packed onto wooden
which are not on the candidate list, exceeding 0.1 pallets, wrapped with steel strapping tape and
percentage by mass: no. strengthened with cardboard corners.
Biocide products were added to this construction
product or it has been treated with biocide products
(this then concerns a treated product as defined by the 2.10 Condition of use
(EU) Ordinance on Biocide Products No. 528/2012): After installation, the boards are resistant to the effects
no. of moisture and will not physically deteriorate when
used in damp or humid conditions. Performance
characteristics are not degraded by age or moisture.
2.6 Manufacture Boards do not encourage mould growth and are
The raw materials are mixed in water and blended in a resistant to attacks by insects or vermin.
reactor to form calcium silicate. This is combined in a
mixer with the other raw materials to form a thick 2.11 Environment and health during use
slurry. The slurry is formed to a board. Boards are When the product is used as designed, the current
dried and edges are trimmed. All material which is cut state of knowledge indicates that there is no risk
off is fully recycled within the production plant. involved for the environment or health.
2.12 Reference service life
The service life according to the "Bundesinstitut für
Bau-, Stadt- und Raumforschung" (BBSR) table is
indicated to be ≥ 50 years.
The reference service life (RSL) is therefore estimated
to be 50 years. This RSL corresponds to the period
after which a building renovation is usually needed,
independently of the actual lifetime of the product
(which can be longer than 50 years).
2.13 Extraordinary effects
Fire
The quality management system of the company and
The boards have a reaction to fire classification A1 or
the production facility are certified according to ISO
non-combustible according to EN13501-1.
9001.
Fire protection
Name Value
2.7 Environment and health during
Building material class A1
manufacturing
Burning droplets -
Promat commits to a clean, healthy and safe working
Smoke gas development -
environment for every person working in and for the
company.
Water
The company and the manufacturing site have an
The boards will not break when exposed to excessive
environment, health and safety management system
amounts of water, e.g. in case of flooding. Since the
which is ISO 14001 and ISO 45001 certified. The
raw materials used are of mineral origin, environmental
manufacturing plant adheres to the Belgium
or health risks are avoided. However, the biological
environmental and health and safety regulations.
and chemical oxygen demand could increase if some
biodegradable components are dissolved in the water.
3 Environmental Product Declaration Etex Building Performance NV – PROMATECT®-100
Mechanical destruction
In order to prevent any reduction of fire performance 2.15 Disposal
following unforeseeable mechanical destruction, all Within the production process, generated waste is re-
damage of the components needs to be repaired using used within the process.
materials specified by ETA 06/0219. When after end-of-life re-using or recycling the boards
Besides the need for repair, the destruction will not as described in the previous paragraph is not practical,
have any significant environmental impact. the boards can be disposed to landfill without pre-
treatment thanks to the largely mineral ingredients
2.14 Re-use phase resulting in an inert matrix, The waste code in
Several possibilities exist for the boards after the end- accordance with the European List of Waste is
of-life of the application in which they were used. 170904.
If the boards are removed non-destructively by
releasing the screws, the undamaged product can be
re-used in accordance with the original purpose. 2.16 Further information
If not contaminated with other building construction Further information is available on the following web
material, the boards also allow being recycled by the site :
manufacturer. https://www.promat.com
Furthermore, the products referred to could be used as
filler and bulk material in civil engineering.
For this EPD, a conservative worst-case scenario was
chosen at the end of life stage and the product was
sent for 100% to landfill.
3. LCA: Calculation rules
3.1 Declared Unit 3.2 System boundary
The declared unit is 1 m² of PROMATECT®-100 with a Type of the EPD: cradle to grave.
thickness of 15 mm. The following life cycle stages and modules are
The results for other thicknesses can be obtained by included:
multiplying the presented results by the corresponding
adjustment factor as included in the table. Production stage (A1-A3):
 pre-chains of the raw materials and their
transportation to the manufacturing site
Declared unit
 energy consumption during production
Name Value Unit
 recycling and disposal of production wastes
Gross density 880 kg/m3
Declared unit 1.00 m²  production of packaging
Grammage 13.2 kg/m²
Conversion factor to 1 kg (divide
results by this factor to obtain the 13.2 - Construction stage (A4-A5):
results for 1 kg)  transportation of product to the construction
Adjustment factor to 1 ton
site
(multiply results by this factor to 75.76 -
 disposal of installation wastes
obtain the results for 1 ton)
Adjustment factor to 1 m² 8 mm  incineration of packaging materials (potential
(multiply results by this factor to 0.53 - benefits from energy substitution within the
obtain the results for 1 m² 8 mm) incineration process are declared in module
Adjustment factor to 1 m² 10 mm D)
(multiply results by this factor to 0.67 -
obtain the results for 1 m² 10 mm)
Adjustment factor to 1 m² 12 mm
Use stage (B1-B7):
(multiply results by this factor to 0.80 -
 efforts for the use of the product,
obtain the results for 1 m² 12 mm)
Adjustment factor to 1 m² 18 mm maintenance and operational efforts
(multiply results by this factor to 1.20 -  modules B3, B4, B5 are declared as MNR
obtain the results for 1 m² 18 mm) (module not relevant) according to the IBU
Adjustment factor to 1 m² 20 mm requirement. These modules are defined on
(multiply results by this factor to 1.33 -
building level in general
obtain the results for 1 m² 20 mm)
Adjustment factor to 1 m² 25 mm
(multiply results by this factor to 1.67 -
obtain the results for 1 m² 25 mm) End-of-life stage (C1-C4):
Adjustment factor to 1 m² 30 mm  transport to disposal of the material
(multiply results by this factor to 2.00 -  landfill end-of-life scenario was considered
obtain the results for 1 m² 30 mm)
Loads and benefits beyond system boundary (D):
 loads and benefits from recycling of
4 Environmental Product Declaration Etex Building Performance NV – PROMATECT®-100
production waste and incineration of 3.6 Data quality
packaging waste This study is mainly based on primary data collected
directly from the manufacturing site and therefore data
quality can be assumed to be very good.
The last update of the GaBi database used for
3.3 Estimates and assumptions
the background data was February 2021.
Most of the input and output influences of the Life
Cycle Inventory Analysis could be depicted using
3.7 Period under review
corresponding data from the GaBi database.
Data for the entire production period of 2019 were
Assumptions and approximations were applied in case
collected and used for this EPD.
of a lack of representative data.
There were no data records in the GaBi database
3.8 Allocation
available for the wooden pallets, they were
Allocation in background data
approximated using the "Solid construction timber"
Specific information on allocation within the
dataset.
background data is given in the GaBi documentation.
The waste water treatment of process water was
Allocation in foreground data
approximated by datasets of municipal waste water
The production process does not deliver any co-
treatment, which will result in an overestimation of
products. In modules A1 to A3, specific raw material
impacts.
and transport data were available, energy, waste and
All assumptions and approximations were documented
water could not be directly allocated to the product and
precisely.
were allocated via the production volume of the
specific products.
3.4 Cut-off criteria
Allocation for waste materials
In the assessment, all utilised raw material, thermal
The environmental burden of the incineration of
energy and electric power were considered
packaging in the construction process stage is
using GaBi datasets. Only the transport of packaging,
assigned to the system (A5); resulting credits for
production waste to recycling/disposal and of
thermal and electrical energy are declared in module
installation loss waste to recycling was cut-off in this
D.
study and one polymeric additive having no
environmental relevance and used at less than 0.1%.
Production of capital equipment, facilities and
3.9 Comparability
infrastructure required for the manufacture are outside
Basically, a comparison or an evaluation of EPD data
the scope of the study and thus were not included.
is only possible if all the data sets to be compared
were created according to EN 15804 and the building
3.5 Background data
context, respectively the product-specific
Background data were sourced from GaBi 10 database
characteristics of performance, are taken into account.
version 2021.
GaBi database version 2021.1 serves as background
database for the calculation of the life cycle
assessment.
4. LCA: Scenarios and additional technical information
No efforts and releases of substances occur during the
normal (i.e. anticipated) use phase.
Transport to the building site (A4)
For the transport from the factory gate to the building
Name Value Unit
site, an average distance of 100km was assumed. This
distance can be assumed to be representative of
Maintenance (B2)
deliveries within Belgium.
No efforts occur during maintenance.
Name Value Unit
Name Value Unit
Litres of fuel 0.028 l/100km
Number/
Transport distance 100 km Maintenance cycle 0 RSL
Capacity utilisation (including 61 % Water consumption 0 m3
empty runs)
Auxiliary 0 kg
Gross density of products
880 kg/m3 Other resources 0 kg
transported
Electricity consumption 0 kWh
Other energy carriers 0 MJ
Material loss 0 kg
Installation into the building (A5)
Only waste treatment of installation loss and packaging
Repair (B3)
is considered in this module.
Name Value Unit
Installation into the building (A5)
Information on the repair process - -
Name Value Unit
Information on the inspection process - -
Material loss 0.66 kg
Number/
VOC in the air 0 kg Repair cycle -
RSL
Water consumption - m3
Auxiliary - kg
Use or application of the installed product (B1) see
Other resources - kg
section 2.12 "Use"
5 Environmental Product Declaration Etex Building Performance NV – PROMATECT®-100
Electricity consumption - kWh Exported electrical energy 1.81 MJ
Other energy carriers - MJ Exported thermal energy 3.26 MJ
Material loss - kg
Replacement (B4) / Refurbishment (B5)
Name Value Unit
Number/
Replacement cycle -
RSL
Electricity consumption - kWh
Litres of fuel - l/100km
Replacement of worn parts - kg
Reference service life
Name Value Unit
Reference service life - a
Life Span (according to BBSR) >=50 a
Life Span according to the
- a
manufacturer
Declared product properties (at the
- -
gate) and finishes
Design application parameters (if
instructed by the manufacturer),
including the references to the - -
appropriate practices and application
codes
An assumed quality of work, when
installed in accordance with the - -
manufacturer’s instructions
Outdoor environment, (for outdoor
applications), e.g. weathering,
pollutants, UV and wind exposure, - -
building orientation, shading,
temperature
Indoor environment (for indoor
applications), e.g. temperature, - -
moisture, chemical exposure
Usage conditions, e.g. frequency of
- -
use, mechanical exposure
Maintenance e.g. required frequency,
type and quality and replacement of - -
components
Operational energy use (B6) and Operational water
use (B7)
No efforts occur in modules B6 and B7.
Name Value Unit
Water consumption 0 m3
Electricity consumption 0 kWh
Other energy carriers 0 MJ
Equipment output 0 kW
End-of-life (C1-C4)
A conservative approach was used in this study.
Although after end-of-life, scenarios where the
boards are re-used or recycled are realistic, a
scenario with 100% landfill was used.
Name Value Unit
Landfilling 13.2 kg
Reuse, recovery and/or recycling potentials (D),
relevant scenario information
Although re-use and recycling of the boards at the end
of life is possible, this is not yet a widely established
practice. Therefore, no possible benefits of recycling or
re-use of the boards were taken into account in this
study. In module D, only the benefits from recycling of
production waste and incineration of waste packaging
were taken into account.
Name Value Unit
6 Environmental Product Declaration Etex Building Performance NV – PROMATECT®-100
5. LCA: Results
The following tables depict the results of the indicators for the Life Cycle Assessment, use of resources and waste
with reference to 1 m² of PROMATECT®-100.
DESCRIPTION OF THE SYSTEM BOUNDARY (X = INCLUDED IN LCA; MND = MODULE NOT DECLARED;
MNR = MODULE NOT RELEVANT)
BENEFITS AND
CONSTRUCTI LOADS
PRODUCT STAGE ON PROCESS USE STAGE END OF LIFE STAGE BEYOND THE
STAGE SYSTEM
BOUNDARIES
7 Environmental Product Declaration Etex Building Performance NV – PROMATECT®-100
lairetam
waR
ylppus tropsnarT
gnirutcafunaM
eht
morf
tropsnarT
etis
eht
ot
etag
ylbmessA esU
ecnanetniaM
riapeR
tnemecalpeR tnemhsibrufeR
ygrene
lanoitarepO esu
retaw
lanoitarepO esu
noitcurtsnoc-eD
noitilomed tropsnarT
gnissecorp
etsaW
lasopsiD -esueR -yrevoceR -gnilcyceR laitnetop
A1 A2 A3 A4 A5 B1 B2 B3 B4 B5 B6 B7 C1 C2 C3 C4 D
X X X X X X X MNR MNR MNR X X X X X X X
RESULTS OF THE LCA - ENVIRONMENTAL IMPACT according to EN 15804+A1: 1 m² 15mm
PROMATECT®-100
Parameter Unit A1 A2 A3 A4 A5 B1 B2 B6 B7 C1 C2 C3 C4 D
GWP [kg CO2-Eq.] 1.46E+01.30E-13.80E+09.02E-21.54E+00.00E+00.00E+00.00E+00.00E+00.00E+04.29E-20.00E+01.89E-1-4.35E-1
9.84E- 2.91E- 1.26E- 2.41E- 4.93E- 1.15E- 1.03E- -6.31E-
ODP [kg CFC11-Eq.] 0.00E+00.00E+00.00E+00.00E+00.00E+0 0.00E+0
10 17 12 17 11 17 15 15
AP [kg SO2-Eq.] 4.08E-3 1.72E-3 3.06E-3 7.17E-5 6.32E-40.00E+00.00E+00.00E+00.00E+00.00E+03.41E-50.00E+01.13E-3-4.79E-4
EP [kg (PO4)3--Eq.] 5.37E-4 2.45E-4 7.46E-4 1.41E-5 1.11E-40.00E+00.00E+00.00E+00.00E+00.00E+06.70E-60.00E+01.28E-4-6.83E-5
POCP [kg ethene-Eq.] 3.57E-4 1.11E-4 4.70E-4-9.06E-76.18E-50.00E+00.00E+00.00E+00.00E+00.00E+0-4.31E-70.00E+08.68E-5-5.00E-5
ADPE [kg Sb-Eq.] 5.54E-7 9.07E-9 6.31E-7 8.14E-9 6.37E-80.00E+00.00E+00.00E+00.00E+00.00E+03.87E-90.00E+01.90E-8-7.29E-8
-
ADPF [MJ] 1.69E+11.69E+07.95E+11.21E+05.33E+00.00E+00.00E+00.00E+00.00E+00.00E+05.75E-10.00E+02.57E+0
6.09E+0
GWP = Global warming potential; ODP = Depletion potential of the stratospheric ozone layer; AP = Acidification potential of land and water; EP =
Caption Eutrophication potential; POCP = Formation potential of tropospheric ozone photochemical oxidants; ADPE = Abiotic depletion potential for non-
fossil resources; ADPF = Abiotic depletion potential for fossil resources
RESULTS OF THE LCA - INDICATORS TO DESCRIBE RESOURCE USE according to EN 15804+A1: 1 m²
15mm PROMATECT®-100
Parameter Unit A1 A2 A3 A4 A5 B1 B2 B6 B7 C1 C2 C3 C4 D
PERE [MJ] 4.65E+0 6.83E-2 7.65E+0 7.03E-2 1.27E+1 0.00E+0 0.00E+0 0.00E+0 0.00E+0 0.00E+0 3.34E-2 0.00E+0 8.05E-1 -1.64E+0
PERM [MJ] 6.07E-1 0.00E+0 1.15E+1 0.00E+0 -1.14E+1 0.00E+0 0.00E+0 0.00E+0 0.00E+0 0.00E+0 0.00E+0 0.00E+0 -4.49E-1 0.00E+0
PERT [MJ] 5.26E+0 6.83E-2 1.92E+1 7.03E-2 1.30E+0 0.00E+0 0.00E+0 0.00E+0 0.00E+0 0.00E+0 3.34E-2 0.00E+0 3.57E-1 -1.64E+0
PENRE [MJ] 1.85E+1 1.71E+0 8.10E+1 1.23E+0 5.56E+0 0.00E+0 0.00E+0 0.00E+0 0.00E+0 0.00E+0 5.83E-1 0.00E+0 2.65E+0 -7.47E+0
PENRM [MJ] 0.00E+0 0.00E+0 2.90E-2 0.00E+0 -2.90E-2 0.00E+0 0.00E+0 0.00E+0 0.00E+0 0.00E+0 0.00E+0 0.00E+0 0.00E+0 0.00E+0
PENRT [MJ] 1.85E+1 1.71E+0 8.10E+1 1.23E+0 5.53E+0 0.00E+0 0.00E+0 0.00E+0 0.00E+0 0.00E+0 5.83E-1 0.00E+0 2.65E+0 -7.47E+0
SM [kg] 1.41E+1 0.00E+0 0.00E+0 0.00E+0 7.05E-1 0.00E+0 0.00E+0 0.00E+0 0.00E+0 0.00E+0 0.00E+0 0.00E+0 0.00E+0 0.00E+0
RSF [MJ] 0.00E+0 0.00E+0 0.00E+0 0.00E+0 0.00E+0 0.00E+0 0.00E+0 0.00E+0 0.00E+0 0.00E+0 0.00E+0 0.00E+0 0.00E+0 0.00E+0
NRSF [MJ] 0.00E+0 0.00E+0 0.00E+0 0.00E+0 0.00E+0 0.00E+0 0.00E+0 0.00E+0 0.00E+0 0.00E+0 0.00E+0 0.00E+0 0.00E+0 0.00E+0
FW [m³] 4.02E-3 7.91E-5 2.27E-2 8.05E-5 4.47E-3 0.00E+0 0.00E+0 0.00E+0 0.00E+0 0.00E+0 3.83E-5 0.00E+0 6.53E-4 -1.63E-3
PERE = Use of renewable primary energy excluding renewable primary energy resources used as raw materials; PERM = Use of
renewable primary energy resources used as raw materials; PERT = Total use of renewable primary energy resources; PENRE = Use of
non-renewable primary energy excluding non-renewable primary energy resources used as raw materials; PENRM = Use of non-
Caption
renewable primary energy resources used as raw materials; PENRT = Total use of non-renewable primary energy resources; SM = Use
of secondary material; RSF = Use of renewable secondary fuels; NRSF = Use of non-renewable secondary fuels; FW = Use of net fresh
water
RESULTS OF THE LCA – WASTE CATEGORIES AND OUTPUT FLOWS according to EN 15804+A1:
1 m² 15mm PROMATECT®-100
Parameter Unit A1 A2 A3 A4 A5 B1 B2 B6 B7 C1 C2 C3 C4 D
HWD [kg] 8.67E-5 6.53E-11 3.30E-8 6.46E-11 4.34E-6 0.00E+0 0.00E+0 0.00E+0 0.00E+0 0.00E+0 3.07E-11 0.00E+0 2.81E-10 -1.65E-9
NHWD [kg] 9.66E-2 2.37E-4 7.14E-1 1.92E-4 7.13E-1 0.00E+0 0.00E+0 0.00E+0 0.00E+0 0.00E+0 9.14E-5 0.00E+0 1.32E+1 -3.69E-3
RWD [kg] 5.19E-4 2.72E-6 5.82E-4 2.22E-6 7.23E-5 0.00E+0 0.00E+0 0.00E+0 0.00E+0 0.00E+0 1.06E-6 0.00E+0 2.78E-5 -5.30E-4
CRU [kg] 0.00E+0 0.00E+0 0.00E+0 0.00E+0 0.00E+0 0.00E+0 0.00E+0 0.00E+0 0.00E+0 0.00E+0 0.00E+0 0.00E+0 0.00E+0 0.00E+0
MFR [kg] 0.00E+0 0.00E+0 8.94E-1 0.00E+0 5.55E-2 0.00E+0 0.00E+0 0.00E+0 0.00E+0 0.00E+0 0.00E+0 0.00E+0 0.00E+0 0.00E+0
MER [kg] 0.00E+0 0.00E+0 0.00E+0 0.00E+0 0.00E+0 0.00E+0 0.00E+0 0.00E+0 0.00E+0 0.00E+0 0.00E+0 0.00E+0 0.00E+0 0.00E+0
EEE [MJ] 0.00E+0 0.00E+0 1.45E-4 0.00E+0 1.81E+0 0.00E+0 0.00E+0 0.00E+0 0.00E+0 0.00E+0 0.00E+0 0.00E+0 0.00E+0 0.00E+0
EET [MJ] 0.00E+0 0.00E+0 3.35E-4 0.00E+0 3.26E+0 0.00E+0 0.00E+0 0.00E+0 0.00E+0 0.00E+0 0.00E+0 0.00E+0 0.00E+0 0.00E+0
HWD = Hazardous waste disposed; NHWD = Non-hazardous waste disposed; RWD = Radioactive waste disposed; CRU = Components
Caption for re-use; MFR = Materials for recycling; MER = Materials for energy recovery; EEE = Exported electrical energy; EET = Exported
thermal energy
6. LCA: Interpretation
The following graph provides information on the
relative contributions of the declared modules to
various environmental impact categories.
It can be observed that for nearly all the impact Transport of the raw materials to site (A2), has in some
categories, the manufacturing (A3), mainly determined of the impact categories such as AP, EP and POCP a
by the energy required for the production process, has fairly important impact (10-25 %).
a very important (25-50 %) or the most important The transport of the product to the building site (A4),
impact (>50 %). Only in the impact category AP and the installation loss and waste treatment of the
ODP, the raw materials have the most important packaging (A5) and the end-of-life modules (C2/C4)
impact. only contribute to a minor extent in most of the impact
The pre-chains of the raw materials (A1) contribute categories.
less than 40% in most of the impact categories and are
mainly linked to impacts caused by the lime and the
fibres.
7. Requisite evidence
table below having "<" means that the measurements
were below the quantification limit)
7.1 Radioactivity measurements Name Value Unit
Radioactivity measurements confirm that no other Total VOC after 28d (C6-C16)
<5 µg/m³
gamma emitters than those originating from natural Limit : 1000
radiation sources are contained. The measured R after 28d (c/NIK) <1 -
radioactivity levels do not exceed the activity Sum of VVOC after 28d (<n-C6) <5 µg/m³
concentration indices as specified by Article 3 Sum of SVOC after 28d (>n-C16)
<5 µg/m³
(Radiation Protection 112) for building products Limit : 100
following the Council Sum of cancerogenic
<1 µg/m³
Directive 96/29. Activity concentration index ≤ 2. Limit : 1
Date: 2 December 2011 Formaldehyd
Measuring agency: SCK.CEN Laboratory for Limit : 120 <3 µg/m³
Gammaspectrometry, Mol, Belgium Acetaldehyd <3 µg/m³
Protocol: Activity concentration index (ACI)
Date: 29 November 2011
Measuring agency: Eurofins Product Testing A/S,
Galten, Denmark
7.2 VOC emissions
Report number: G10210A
VOC measurements confirmed compliance with the
requirements of DIBt DIBt-communication 4/2004 in
combination with the NIK values from AgBB (March
2008) for use in the indoor environment. (values in the
8 Environmental Product Declaration Etex Building Performance NV – PROMATECT®-100
8. References
Standards
BBSR
EN 826 BBSR table "Service lives of components for life cycle
EN 826: 1996: Thermal insulating products for building assessment according to Bewertungssystem
applications - Determination of compression behaviour Nachhaltiges Bauen (BNB)" Sustainable Building
Information Portal by the Federal Ministry of Transport,
EN 1607 Building and Urban Affairs (Bundesinstitut für Bau-
EN 1607: 1996: Thermal insulating products for ,Stadt-und Raumforschung, BBSR).
building applications - Determination of tensile strength (https://www.nachhaltigesbauen.de/baustoff-
perpendicular to faces undgebaeudedaten/
nutzungsdauern-von-bauteilen.html)
EN 1608
EN 1608: 1996: Thermal insulating products for Candidate list
building applications - Determination of tensile strength Candidate List of substances of very high concern for
parallel to faces Authorisation, published on ECHA website, latest
version 19.01.2021. (https://echa.europa.eu/candidate-
EN 12467 list-table).
EN 12467: 2004: Fibre-cement flat sheets - Product
specification and test methods CPR
Construction Products Regulation, Regulation (EU) No
EN 12667 305/2011 of the European Parliament and of the
EN 12667: 2001: Thermal performance of building Council of 9 March 2011 layingdown harmonized
materials and products- Determination of thermal conditions for the marketing of construction products
resistance by means of guarded hot plate and heat and repealing Council Directive 89/106/ EEC Text with
flow meter methods. Products of high and medium EEA relevance.
thermal resistance.
DIBt-communication 4/2004
EN 13501-1 DIBt (Deutsches Institut für Bautechnik) approval
EN 13501-1:2018, Fire classification of construction guidelines for the health-related evaluation of indoor
products and building elements - Part 1: Classification construction products-2004.
using data from reaction to fire tests.
Directive 96/29
EN 15804 Council Directive 96/29/Euratom of 13 May 1996 laying
EN 15804:2012+A2:2019, Sustainability of down basic safety standards for the protection of the
construction works — Environmental Product health of workers and the general public against the
Declarations — Core rules for the product category of dangers arising from ionising radiation.
construction products.
European List of Waste
ISO 9001 2014/955/EU: Commission Decision of 18 December
UNI EN ISO 9001:2015 September 2015, Quality 2014 amending Decision 2000/532/EC on the list of
management systems - Requirements waste pursuant to Directive 2008/98/EC of the
European Parliament and of the Council.
ISO 12572 (http://data.europa.eu/eli/dec/2014/955/oj)
DIN EN ISO 12572:2001, Hygrothermal performance
of building materials and products - Determination of ETA 06/0219
water vapour transmission properties - Cup method European technical approval of PROMATECT®-100
fire protective board.
ISO 14001
UNI EN ISO 14001:2015, Environmental management Eurofins Product Testing A/S
systems - Requirements with guidance for use. Eurofins Product Testing A/S, Smedeskovvej 38, 8464
Galten, Denmark. Report number: G10210A; 2011.
ISO 14025
DIN EN ISO 14025:2011-10, Environmental labels and GaBi
declarations — Type III environmental declarations — GaBi Software System and Database for Life Cycle
Principles and procedures. Engineering, 1992-2021, Sphera Solutions GmbH,
Leinfelden-Echterdingen, with acknowledgement of
ISO 45001 LBP University of Stuttgart, program version GaBi 10;
ISO 45001:2018, Occupational health and safety database version 2021.1.
management systems — Requirements with guidance
for use GaBi documentation
GaBi dataset documentation for the software system
Further References and databases, LBP, University of Stuttgart and
Sphera Solutions GmbH, Leinfelden-Echterdingen,
AgBB 2021.
Ausschuss zur gesundheitlichen Bewertung von (http://www.gabi-software.com/support/gabi/gabi-
Bauprodukten, AgBB (eng. German Committee for database-2021-lci-documentation/)
health-related evaluation of building products.
9 Environmental Product Declaration Etex Building Performance NV – PROMATECT®-100
IBU 2021 insulating materials, version 1.6, 2017 www.bau-
Institut Bauen und Umwelt e.V.: General Programme umwelt.de
Instructions for the Preparation of EPDs at the Institut
Bauen und Umwelt e.V. Version 2.0, Berlin: Institut REACH Regulation
Bauen und Umwelt e.V., 2021. Regulation (EU) No 1907/2006 of the European
(http://www.ibu-epd) Parliament and of the Council of 18 December 2006
concerning the Registration, Evaluation, Authorisation
Ordinance on Biocide Products and Restriction of Chemicals (REACH), establishing a
Regulation (EU) No 528/2012 of the European European Chemicals Agency, amending Directive
Parliament and of the Council of 22 May 2012 1999/45/EC and repealing Council Regulation (EEC)
concerning the making available on the market and No 793/93 and Commission
use of biocidal products. Regulation (EC) No 1488/94 as well as Council
Directive 76/769/EEC and Commission Directives
PCR Part A 91/155/EEC, 93/67/EEC, 93/105/EC and 2000/21/EC.
PCR Part A: Calculation rules for the Life Cycle
Assessment and Requirements on the Background SCK CEN Laboratory
Report according to EN 15 804+A2:2019, Version 1.0, Belgian Nuclear Research Centre in Mol.
Institut Bauen und Umwelt e.V., 2020.
PCR Part B
Product Category Rules for Building Products, Part B :
Requirements on the EPD for Calcium silicate
10 Environmental Product Declaration Etex Building Performance NV – PROMATECT®-100
Publisher
Institut Bauen und Umwelt e.V. Tel +49 (0)30 3087748- 0
Panoramastr. 1 Fax +49 (0)30 3087748- 29
10178 Berlin Mail info@ibu-epd.com
Germany Web www.ibu-epd.com
Programme holder
Institut Bauen und Umwelt e.V. Tel +49 (0)30 - 3087748- 0
Panoramastr 1 Fax +49 (0)30 – 3087748 - 29
10178 Berlin Mail info@ibu-epd.com
Germany Web www.ibu-epd.com
Author of the Life Cycle
Assessment Tel +32 (0)15 71 82 83
Peggy Van De Velde Fax +32 (0)15 71 82 29
Bormstraat 24 Mail
2830 Tisselt peggy.vandevelde@etexgroup.c
Belgium om
Web www.etexgroup.com
Owner of the Declaration
Etex Building Performance Tel +32 2 778 12 11
International Fax +32 2 778 12 12
Rue Marcel Demonque 500 r Mail info@etexgroup.com
84915 Avignon Cedex 9 Web http://www.etexgroup.com
France
