ENVIRONMENTAL PRODUCT DECLARATION
as per ISO 14025 and EN 15804+A1
Owner of the Declaration NMC S.A.
Programme holder Institut Bauen und Umwelt e.V. (IBU)
Publisher Institut Bauen und Umwelt e.V. (IBU)
Declaration number EPD-NMC-20210309-IBD1-EN
Issue date 05.01.2022
Valid to 04.01.2027
CLIMAFLEX®naturefoam exzentro
NMC S.A.
www.ibu-epd.com | https://epd-online.com
Umwelt Produktdeklaration Name des Herstellers – Name des Produkts
1. General Information
NMC S.A. CLIMAFLEX®naturefoam exzentro
Programme holder Owner of the declaration
IBU – Institut Bauen und Umwelt e.V. NMC S.A.
Panoramastr. 1 Gert-Noel Strasse
10178 Berlin BE-4731 Eynatten
Germany
Declaration number Declared product / declared unit
EPD-NMC-20210309-IBD1-EN 1 m³ insulation material CLIMAFLEX®naturefoam
exzentro
This declaration is based on the product Scope:
category rules: Product line CLIMAFLEX®naturefoam exzentro
Insulating materials made of foam plastics, 01.2019 Thermal insulation products for building equipment and
(PCR checked and approved by the SVR) industrial insulations made of Polyethylene-based,
closed-cell foam pipe insulation with a robust protective
Issue date coating (PEF) according to /EN14313/. This declaration
is an Environmental Product Declaration according to
05.01.2022
/ISO14025/ describing the specific environmental
performance of the product produced in Belgium at the
Valid to
site of Eynatten. CLIMAFLEX®naturefoam exzentro is
04.01.2027 rectangular and thus more suitable for the insulation of
heating pipes in a concrete floor
The owner of the declaration shall be liable for the
underlying information and evidence; the IBU shall not
be liable with respect to manufacturer information, life
cycle assessment data and evidences.
The EPD was created according to the specifications
of EN 15804+A1. In the following, the standard will be
simplified as EN 15804.
Verification
The standard EN 15804 serves as the core PCR
Independent verification of the declaration and data
according to ISO 14025:2010
Dipl. Ing. Hans Peters internally x externally
(chairman of Institut Bauen und Umwelt e.V.)
Dr. Alexander Röder Vito D'Incognito
(Managing Director Institut Bauen und Umwelt e.V.)) (Independent verifier)
2. Product
2.1 Product description/Product definition  Products made of PE foam yield an excellent
CLIMAFLEX®naturefoam exzentro is the Professional cost/performance ratio.
Polyethylene-based closed-cell foam pipe insulation
 Heat loss control and noise reduction in fresh-
with a robust PE protective coating for continued
and waste water and heating systems
energy saving and condensation control purposes.
CLIMAFLEX®naturefoam exzentro with its rectangular
and thin design, it is used in flooring.
For the placing on the market of the product in the 2.3 Technical Data
European Union/European Free Trade Association
(EU/EFTA) (with the exception of Switzerland) -
Thermal Insulation products for building equipment and Constructional data
industrial installations. Factory made polyethylene Name Value Unit
foam (PEF) and the CE-marking. For the application Gross density 34.2 kg/m3
and use, the respective national provisions apply. 0.04 -
Thermal conductivity W/(mK)
2.2 Application 0.042
CLIMAFLEX®naturefoam exzentro is used in flooring Reaction to fire acc.to /EN 13501-
E -
 Polyethylene foam is a cost-efficient material 1/
with good insulating properties. Max Service Temperature acc. To
100 °C
/EN14706/, /EN 14707
2 Environmental Product Declaration NMC sa – CLIMAFLEX®naturefoam exzentro
Min Service Temperature 0 °C Antimony trioxide and halogenated flame retardants
Water absorption acc. to /EN are applied.
WS005
13472/
Traces quantities of water soluble Cl < 20 – F
ions and pH-value acc. to EN < 4 - pH
13468 and EN 13472 5,8 2.6 Manufacture
The manufacturing process consists of a continuous
extrusion. Solid pellets of thermoplastic resin are fed to
a melting zone in which the resin is melted, to form a
flowable thermoplastic mass. The thermoplastic mass
2.4 Delivery status is then metered to a mixing zone where the
The PE products are supplied as tubes. The tubes are thermoplastic mass is thoroughly mixed with a blowing
delivered in lengths of 2 m packed in cardboard boxes. agent under pressure. The mixture of thermoplastic
The insulating sleeves in the CLIMAFLEX®naturefoam resin and blowing agent is then forced through a die,
exzentro have a thickness ranging from 9 to 51mm and which imparts a shape to the thermoplastic mass, into
an inside diameter ranging from 15 to 42mm. These a zone of lower pressure, such as atmospheric
products are categorized according to thermal pressure. The blowing agent expands to form the cells
conductivity (Lambda*). The category of product with of the foam and the thermoplastic foam is cooled
lambda 0,040 (W/(mK)) (acc. to /EN ISO 8497/ and trough an inline water cooler. The protection coating
/EN 12667/) includes CLIMAFLEX®naturefoam "skin" is applied by co-extrusion. The "skin" is made
exzentro with thickness 9 mm, while the category of with solid pellets of thermoplastic resin and some
product with lambda 0,042 (W/(mK)) (acc. to /EN additives, which is, with the help of an extruder,
12667/) includes CLIMAFLEX®naturefoam applied around the foam. There is no a foaming agent
exzentro with thicknesses from 25 to 51mm products. used in this case. The die is positioned around the
"naked" foam and deposes a small thickness (± 0.1
2.5 Base materials/Ancillary materials mm) of PE film on the foam. At the end of this process
the profiles are cut at dimension.
Base materials
CLIMAFLEX®naturefoam exzentro is a flexible Quality assurance :
insulation material based on Polyethylene with a The manufacture is certified /ISO 9001/ for the quality
protecting coating of PE., which consists of around 8 management. The product corresponds to the product
basic components. The following table displays the standard /EN 14313/ and has a Declaration of
different elements of formula. Performance according to the /CPR/ : DOP no.
This product contains substances listed in the W1PEF300 ; W1PEF400 (see www.nmc-
candidate list (date: 08.07.2021) exceeding 0.1 insulation.com)
percentage by mass: No.
This product contains other CMR substances in
categories 1A or 1B which are not on the candidate 2.7 Environment and health during
list, exceeding 0.1 percentage by mass: No. manufacturing
Biocide products were added to this construction During all manufacturing steps of NMC S.A. Belgium,
product or it has been treated with biocide products the production follows the national guidelines and
(this then concerns a treated product as defined by the regulations. Solar panels are installed on the roof of
(EU) Ordinance on Biocide Products No. 528/2012): the warehouses.
No.
2.8 Product processing/Installation
CLIMAFLEX®naturefoam exzentro can be installed
using basic tools like knives. No special tools, or
specific protection is necessary. When applying
Name Value Unit adhesives the information given in the relevant safety
BIO LDPE 52,06 % data sheets is to be heeded.The recommendations on
Polyethylene 11,55 % how to use the product is described in the application
NMC Internally recycled PE 22,41 % manuals or video's. More details are listed on the Web
Flame retardant 3,92 % Page www.nmc-insulation.com
Pigments and fillers 3,02 %
Volume stabilizer 0,97 % 2.9 Packaging
Blowing Agent 6,07 % CLIMAFLEX®naturefoam exzentro products are
packed in cardboard boxes and transported on
PE and fillers give the aspect of the product. The reusable pallets. The packaging material can be
blowing agent causes the expansion during recycled.The pallets used to transport the products are
manufacturing. And the flame retardants ensure the taken back or exchanged when the
fire resistance. According the European Chemicals CLIMAFLEX®naturefoam easy is delivered, so the use
Regulation /REACH/ Manufacturers, importers and of pallets is a close loop economy.
downstream users must register their chemicals and
are responsible for their safe use on their own. For its
production NMC S.A. uses exclusively verifiably
registered and approved substances. Products 2.10 Condition of use
manufactured and put on the market by NMC need to During the use of the product for the purpose for
be registered. CLIMAFLEX®naturefoam exzentro does which they are intended, there are no modifications on
not contain Substances of Very High Cincern (SVHC). the product during the use, except if due to
extraordinary impact (see point 2.13).
3 Environmental Product Declaration NMC sa – CLIMAFLEX®naturefoam exzentro
2.11 Environment and health during use therefore have a limited speed of inflammation.
There are no particular aspects of the material
composition during the use. CLIMAFLEX®naturefoam
exzentro products are used in a wide range and
varieties of applications for which the product is Fire Protection
intended to. The PEF foams fulfil the German, Belgian Name Value
and French regulations regarding the emission of VOC Building material class E
with emissions far below the most severe limit values.
The Eurofin Product Testing institute, on the demand Water
of the CEFEP (European group of PEF and FEF CLIMAFLEX®naturefoam exzentro are closed cell
manufacturers) has made a wide range of tests for foam and obtain the better water absorption class
different PEF products from different manufacturers. WS005 according to the product standard
The insulation of heating pipes with
CLIMAFLEX®naturefoam exzentro allows a reduction Mechanical destruction
of energy dispersion and, of course CO emission CLIMAFLEX®naturefoam exzentro are flexible foam
2
during the full service life of the installation. The covered with a PE protective coating
quantification of this is not in the topic of this EPD, and CLIMAFLEX®naturefoam exzentro are not UV
has to be evaluated in the frame of the LCA from the resistant. The use is not recommended for outside
complete installation applications without complementary UV protection.
2.12 Reference service life 2.14 Re-use phase
The function of CLIMAFLEX®naturefoam exzentro is In principle, if removed carefully,
to ensure the insulation of heating and sanitary CLIMAFLEX®naturefoam exzentro can be reused on
installations for a reference service life (RSL) of 50 any other piping system of similar dimensions. Any
years. This duration is based on the frequency of material not suitable for reuse is fully recyclable.
replacement of sanitary and heating piping in buildings.
Although the insulation products are still effective after 2.15 Disposal
50 years, it is assumed that when replacing the piping, CLIMAFLEX®naturefoam exzentro are fully recyclable
the insulation CLIMAFLEX®naturefoam exzentro is not using the same recycling systems as those used for
reused and is disposed of with the piping. 50 years is other forms of PE waste.
the minimum Reference Service Life recommended in Any non-recycled material should be disposed of the
/EN16783/ . materials according to the local regulations, and by the
/European Waste Catalogue waste code 07 02 13
waste Plastic "Low Density Polyethylene"
2.13 Extraordinary effects
2.16 Further information
Fire Additional information about CLIMAFLEX®naturefoam
According to EN13501-1 CLIMAFLEX®naturefoam exzentro can be found on the NMC web site www.nmc-
exzentro are classified as EURO CLASS E and insulation.com Here specification clauses, data sheets
and application manuals can be found.
3. LCA: Calculation rules
3.1 Declared Unit depending on the pipe diameter.
The declaration refers to 1 m³ of produced insulation
product. For the LCA calculations, as the product is For IBU core EPDs (where clause 3.6 is part of the
foam and have some tolerances, the density declared EPD): for average EPDs, an estimate of the
is the average between the product categories. The robustness of the LCA values must be made, e.g.
thermal conductivity coefficient (Lambda-value) and R- concerning variability of the production process,
value per 25 mm thickness per product brand is geographical representativeness and the influence of
provided below as additional information and support background data and preliminary products compared
for installers. to the environmental impacts caused by actual
production.
Name Value Unit
Declared unit 1 m3 3.2 System boundary
Gross density 34.2 kg/m3 The Data collection refers to the yearly production in
Volume for 1kg 0,02924 kg 2020.
Value for 1 Module A1 to A3:The raw material data used for
m3 CLIMAFLEX®naturefoam exzentro are derived from
divided the GaBi 2021 life cycle database used in the GaBi 10
Conversion factor from 1m³ to 1
section of m software environment (Service Pack 2021001000).
meter
the Where data were missing or were unavailable or where
insulation suppliers were unable to provide complete information,
pipe ( m²) proxy datasets have been used. Where data is missed,
like some component of volume stabilizer, (the correct
Thermal Conductivity λ: 0.040 W/mK at (40°C) data is not in GaBi software) we use proxy datasets. It
R-value- thickness: 25 mm: +/- 3,5 (m²K)/W concerns the volume stabilizers, the orange colour and
Thermal Conductivity λ: 0.042 W/mK at (40°C) the Pigment EMP. For some raw material produced by
R-value- thickness: 25 mm: +/- 3,355 (m²K)/W the external supplier (Volume stabilizer, colour) the
manufacture of the CLIMAFLEX®naturefoam exzentro
4 Environmental Product Declaration NMC sa – CLIMAFLEX®naturefoam exzentro
product consists of incorporating the ingredients of the Module C3: The scenario that has been retained for
formulation into an extruder, adding a foaming agent, this Life Cycle Assessment is the 100% recycling
mixing, heating and then extruding the mix through a Module C4: As CLIMAFLEX®naturefoam exzentro is
die, during which time foaming takes place. The fully recyclable, the legislation is pushing more in this
product is then cooled with water (municipal water), direction and the overall pressure on plastic recycling
drying and the skin (Bio-LDPE not foamed) is applied. is growing, therefore the scenario with 100% recycling
After that, the product is cut to size before being is considered.
packed and stored. The production waste from the Module D: The end-of-life scenarios for packaging
process (regenerate in the GaBi model) (machine start, material and product do not deliver any benefits for the
end of production, non-conforming products, etc.) is next system. The recycling of cardboard is a closed
recycled internally (on a dedicated machine for this cycle with the production process. The
purpose) in order to be reused in the manufacturing CLIMAFLEX®naturefoam exzentro foam is fully
process. . All production takes place exclusively in recyclable and can be used as a direct one-for-one
Eynatten, Belgium. substitute for virgin PE-LD granulates, with only minor
Module A4: The type of transport included in the LCA additive additions. There is no chemical difference
model is a truck mix Euro Cargo 0-6 with diesel fuel. between bio-based PE-LD and fossil fuel derived PE-
As the product is foam with a comparatively low LD, so using a mix of sources does not change the
density, the product volume is the limiting factor on recyclability of the product.
loading. CLIMAFLEX®naturefoam exzentro is rarely
the only product loaded in trucks, they are usually 3.3 Estimates and assumptions
grouped with other products of higher density The LCA calculation is conducted using the Gabi ts -
according to the place of destination. In addition, NMC database. Not all necessary LCIs are included in the
s.a. works with regional expeditions companies that database. Where data were missing or were
group different goods in order to optimize the weight- unavailable or where suppliers were unable to provide
to-volumes ratio. For this reason, the fill rate of the complete information, proxy datasets have been used.
trucks has been set to 10% of the mass payload The environmental burden for the production of
capacity. pigments, flame retardants and volume stabilizers are
Module A5: Installation of CLIMAFLEX®naturefoam approximated.
exzentro products is done by hand and requires no
special equipment apart from a knife. The products can 3.4 Cut-off criteria
be placed end to end and the remaining pieces can be Any glue and adhesive tapes used during the
reused. Some glue or tape could be used for the installation (A5) have not been included as
installation, as the quantity or the product used quantification of these materials is uncertain and their
depends of the final customer, he has to calculate the use by the various installers is too diverse, adhesives
impact of what he used himself. The environmental and glues are not required in all/most cases, but may
impact of this type of accessories are not counted in be used for some applications.
this study. The calculations do not contain any In this study no others cut-off criteria have been
installation waste. Cardboard as packaging material is applied and all elementary incoming processes as well
assumed to be recycled. As input material cardboard as all energy and water inputs and waste outputs have
made of waste paper is considered. Thus, been counted.
environmental burden for packaging material are
considered already in A1-A3. The value of the 3.5 Background data
environmental impact for A5 is declared as “0”. The The software system for life cycle engineering GaBi 10
choice made is : the final user has to calculate the developed by Thinkstep AG was used to perform this
impact of A5 himself in function of his own case, by LCA. The GaBi 10 software environment (Service Pack
accounting for the extra amount of product needed 2021001000) provides the life cycle inventory data for
during installation. several of the raw and process materials obtained from
Module B1-B7:Once installed the the background system.
CLIMAFLEX®naturefoam exzentro product requires no
maintenance and no repair. It will be dismantled when 3.6 Data quality
the sanitary pipe is replaced. For this reason, there are All the foreground data requiring such energy or raw
not expected to be any impacts in B1 to B7 assuming material coming from production, were verified and
correct specification and installation. The step B1 is not cross-checked before being included in the model.
considered in this LCA, although the insulation of the Most of the life cycle inventories for the basic materials
piping contributes to a significant reduction of CO are available in the GaBi 10 software environment
2
emissions from the heating or cooling equipment, this (Service Pack 2021001000) database.
is not taken into account in this LCA. It should, For electrical and thermal energy Belgium specific grid
however, be taken into account in the calculation of mixes and Belgium specific supply for natural gas were
environmental impacts of the complete heating and considered.
cooling systems or of the complete building.
Module C1:As for the installation of the product, the 3.7 Period under review
disassembly is done manually and does not require The production data for the year 2020 were used for
any specific equipment. Disassembly is generally the realisation of this study.
carried out at the same time as the replacement or
removal of sanitary pipes. Consequently, there are no 3.8 Allocation
impacts associated with C1. There is no co-product or by-product generated during
Module C2:Transport at end-of-life stage is modeled the production of NMC’s products.
as a Euro Cargo 0-6 mix truck with diesel fuel. The Due to the lack of specific data per production line and
average distance to either mechanical recycling is product, the energy has been allocated per overall
assumed to be 100 km. produced volume of insulation foam.
5 Environmental Product Declaration NMC sa – CLIMAFLEX®naturefoam exzentro
Production waste 3.9 Comparability
Most of the production waste from the process Basically, a comparison or an evaluation of EPD data
(machine start, end of production, non-conforming is only possible if all the data sets to be compared
products, etc.) is recycled internally in order to be were created according to EN 15804 and the building
reused in the manufacturing process. These impacts context, respectively the product-specific
are accounted for in A1-A3. characteristics of performance, are taken into account.
Installation and End-of-Life waste
Installation of the foam products is done by hand and
requires no special equipment apart from a knife.
Installation off-cut is not considered in this calculations.
Any glue and adhesive tapes used during the
installation phase were not included in the LCA.
4. LCA: Scenarios and additional technical information
Electricity consumption - kWh
Litres of fuel - l/100km
Transport to the building site (A4) Replacement of worn parts - kg
Name Value Unit
Litres of fuel 0.167 l/100km
Transport distance 445 km Reference service life
Capacity utilisation (including Name Value Unit
10 %
empty runs) Reference service life 50 a
Gross density of products
34.2 kg/m3
transported Operational energy use (B6) and Operational water
use (B7)
Installation into the building (A5) Name Value Unit
The calculations do not contain any installation waste. Water consumption - m3
Cardboard as a packaging material is assumed to be Electricity consumption - kWh
recycled. As input material cardboard made of waste Other energy carriers - MJ
paper is considered. Thus, the environmental burden Equipment output - kW
for packaging material is considered already in A1-A3.
The value of the environmental impact for A5 is End of life (C1-C4)
declared as “0”. The choice made is : the final user has Name Value Unit
to calculate the impact of A5 himself in the function of Recycling 34.2 kg
his own case, by accounting for the extra amount of
product needed during installation. Reuse, recovery and/or recycling potentials (D),
Name Value Unit relevant scenario information
Name Value Unit
Use or application of the installed product (B1) see
section 2.12 "Use"
Name Value Unit
Maintenance (B2)
Name Value Unit
Auxiliary - kg
Other energy carriers - MJ
Material loss - kg
Repair (B3)
Name Value Unit
Information on the repair process - -
Information on the inspection process - -
Number/
Repair cycle -
RSL
Water consumption - m3
Auxiliary - kg
Other resources - kg
Electricity consumption - kWh
Other energy carriers - MJ
Material loss - kg
Replacement (B4) / Refurbishment (B5)
Name Value Unit
Number/
Replacement cycle -
RSL
6 Environmental Product Declaration NMC sa – CLIMAFLEX®naturefoam exzentro
5. LCA: Results
DESCRIPTION OF THE SYSTEM BOUNDARY (X = INCLUDED IN LCA; MND = MODULE NOT DECLARED;
MNR = MODULE NOT RELEVANT)
BENEFITS AND
CONSTRUCTI LOADS
PRODUCT STAGE ON PROCESS USE STAGE END OF LIFE STAGE BEYOND THE
STAGE SYSTEM
BOUNDARIES
7 Environmental Product Declaration NMC sa – CLIMAFLEX®naturefoam exzentro
lairetam
waR
ylppus tropsnarT
gnirutcafunaM
eht
morf
tropsnarT
etis
eht
ot
etag
ylbmessA esU
ecnanetniaM
riapeR
tnemecalpeR tnemhsibrufeR
ygrene
lanoitarepO esu
retaw
lanoitarepO esu
noitcurtsnoc-eD
noitilomed tropsnarT
gnissecorp
etsaW
lasopsiD -esueR -yrevoceR -gnilcyceR laitnetop
A1 A2 A3 A4 A5 B1 B2 B3 B4 B5 B6 B7 C1 C2 C3 C4 D
X X X X X MND MND MNR MNR MNR MND MND MND X X X X
RESULTS OF THE LCA - ENVIRONMENTAL IMPACT according to EN 15804+A1: 1 m³
CLIMAFLEX®naturefoam exzentro
Parameter Unit A1-A3 A4 A5 C2 C3 C4 D
GWP [kg CO2-Eq.] 24.25 1.74 0.00 0.29 3.11 0.00 -87.91
ODP [kg CFC11-Eq.] 8.43E-8 4.67E-16 0.00E+0 7.68E-17 2.80E-13 0.00E+0 -1.17E-12
AP [kg SO2-Eq.] 1.08E+0 1.49E-3 0.00E+0 2.46E-4 3.22E-3 0.00E+0 -1.00E-1
EP [kg (PO4)3--Eq.] 9.38E-1 2.99E-4 0.00E+0 4.92E-5 7.81E-4 0.00E+0 -1.58E-2
POCP [kg ethene-Eq.] 2.74E-1 1.94E-4 0.00E+0 3.20E-5 3.73E-4 0.00E+0 -1.78E-2
ADPE [kg Sb-Eq.] 2.77E-1 1.57E-7 0.00E+0 2.59E-8 2.31E-6 0.00E+0 -2.13E-5
ADPF [MJ] 1693.46 23.38 0.00 3.85 41.32 0.00 -3402.86
GWP = Global warming potential; ODP = Depletion potential of the stratospheric ozone layer; AP = Acidification potential of land and water; EP =
Caption Eutrophication potential; POCP = Formation potential of tropospheric ozone photochemical oxidants; ADPE = Abiotic depletion potential for non-
fossil resources; ADPF = Abiotic depletion potential for fossil resources
RESULTS OF THE LCA - INDICATORS TO DESCRIBE RESOURCE USE according to EN 15804+A1: 1 m³
CLIMAFLEX®naturefoam exzentro
Parameter Unit A1-A3 A4 A5 C2 C3 C4 D
PERE [MJ] 2230.61 1.36 0.00 0.22 41.82 0.00 -214.05
PERM [MJ] 1330.06 0.00 0.00 0.00 0.00 0.00 0.00
PERT [MJ] 3560.67 1.36 0.00 0.22 41.82 0.00 -214.05
PENRE [MJ] 1747.09 23.71 0.00 3.90 125.19 0.00 -3473.87
PENRM [MJ] 358.02 0.00 0.00 0.00 0.00 0.00 0.00
PENRT [MJ] 2105.11 23.71 0.00 3.90 125.19 0.00 -3473.87
SM [kg] 12.55 0.00 0.00 0.00 0.00 0.00 0.00
RSF [MJ] 0.00 0.00 0.00 0.00 0.00 0.00 0.00
NRSF [MJ] 0.00 0.00 0.00 0.00 0.00 0.00 0.00
FW [m³] 0.30 0.00 0.00 0.00 0.03 0.00 -0.39
PERE = Use of renewable primary energy excluding renewable primary energy resources used as raw materials; PERM = Use of
renewable primary energy resources used as raw materials; PERT = Total use of renewable primary energy resources; PENRE = Use of
non-renewable primary energy excluding non-renewable primary energy resources used as raw materials; PENRM = Use of non-
Caption
renewable primary energy resources used as raw materials; PENRT = Total use of non-renewable primary energy resources; SM = Use
of secondary material; RSF = Use of renewable secondary fuels; NRSF = Use of non-renewable secondary fuels; FW = Use of net fresh
water
RESULTS OF THE LCA – WASTE CATEGORIES AND OUTPUT FLOWS according to EN 15804+A1:
1 m³ CLIMAFLEX®naturefoam exzentro
Parameter Unit A1-A3 A4 A5 C2 C3 C4 D
HWD [kg] 7.36E-4 1.25E-9 0.00E+0 2.06E-10 4.28E-8 0.00E+0 -5.11E-7
NHWD [kg] 1.21E+1 3.72E-3 0.00E+0 6.12E-4 1.37E-1 0.00E+0 -9.48E-1
RWD [kg] 1.33E-1 4.30E-5 0.00E+0 7.07E-6 3.30E-2 0.00E+0 -2.66E-2
CRU [kg] 0.00 0.00 0.00 0.00 0.00 0.00 0.00
MFR [kg] 0.00 0.00 12.55 0.00 48.20 0.00 0.00
MER [kg] 0.00 0.00 0.00 0.00 0.00 0.00 0.00
EEE [MJ] 0.00 0.00 0.00 0.00 0.00 0.00 0.00
EET [MJ] 0.00 0.00 0.00 0.00 0.00 0.00 0.00
HWD = Hazardous waste disposed; NHWD = Non-hazardous waste disposed; RWD = Radioactive waste disposed; CRU = Components
Caption for re-use; MFR = Materials for recycling; MER = Materials for energy recovery; EEE = Exported electrical energy; EET = Exported
thermal energy
6. LCA: Interpretation
The base polymer used at NMC is produced from 80% of the impact Global Warming Potential. As the
renewable raw materials (Biomass/Sugar cane). One CLIMAFLEX® naturefoam exzentro is fully recyclable;
of the advantages of using a biopolymer is a significant the choice for the end of life was that of 100%
reduction in greenhouse gas emissions compared to recycling. This avoids the use of new raw materials
the use of raw materials of fossil origin. In addition, the and or the exploitation of renewable or non-renewable
use of non-renewable raw materials is avoided in this resources. One way to continue to reduce the
way. When we analyse the complete life cycle we see environmental impact of the CLIMAFLEX® naturefoam
that the most impacting part for all environmental exzentro would be to continue to diversify our energy
impact factors is the production module and more sources by switching more and more to renewable
particularly the raw materials. With regard to global energies. To this end, after having greatly increased
warming for the complete life cycle, more than 78% the number of photovoltaic panels, NMC will acquire a
comes from the production module 1,4 % of transport cogeneration system. Looking for more eco-
to the places of installation and 12,4% comes from the responsible suppliers must also be put in place, as well
end of life. For all other impact factors, more than 90% as finding raw materials manufactured locally to avoid
of the impacts come from the production phase. long-distance transport as much as possible. An
Transport has a more pronounced impact on global analysis of the plant's carbon footprint, which is
warming potential as well as on soil and water currently being carried out, should enable NMC to
acidification potential and abiotic fossil resource identify areas for improvement and find solutions to
depletion potential. A more in-depth analysis of the achieve the goal of zero carbon.
production module A1 to A3 shows that the production
of raw materials and their transport account for most of
7. Requisite evidence
7.1. VOC emissions VOC Emissions
Eurofins Product Testing A/S has tested a wide range Name Value Unit
and variety of typical PEF (Polyethylene foam) Overview of Results (28 Tage) - μg/m3
products marketed in the EU from CEFEP (European TVOC (C6 - C16) - μg/m3
Group of PEF/FEF manufacturers) Based on the Sum SVOC (C16 - C22) - μg/m3
loading factor 0.05m²/m3 (determined after R (dimensionless) - -
consideration of the real life applications of PEF VOC without NIK - μg/m3
products (in living rooms) and recommendations by the Carcinogenic Substances - μg/m3
experts of the test institute) all results were found to be
clearly below the limit values. For all samples below AgBB overview of results (3 days [µg/m³])
100mg/m3 TVOC after 28 days. Certificates are
Name Value Unit
available on request. TVOC (C6 - C16) - μg/m3
Sum SVOC (C16 - C22) - μg/m3
7.2 Leaching
R (dimensionless) - -
According to /EN 13468/ the content of water-soluble
VOC without NIK - μg/m3
chloride ions for CLIMAFLEX®naturefoam exzentro is
Carcinogenic Substances - μg/m3
<20 mg/kg.
8. References
EN 1602 ISO 14001
EN 1602: 2013: Thermal insulating products for ISO 14001: 2015 Environmental management
building applications - Determination of the apparent systems.
density
EN ISO 14025
EN ISO 8497 EN ISO 14025: 2011-10: Environmental labels and
EN ISO 8497: Thermal insulation - Determination of declarations — Type III environmental declarations —
steady-state thermal transmission properties of thermal Principles and procedures
insulation for circular pipes
ISO 14040
ISO 9001 ISO 14040: Environmental management — Life cycle
ISO 9001: 2015: Quality management systems. assessment — Principles and framework
EN 13501-1 ISO 14044
EN 13501-1:2007+A1: 2013 Fire classification of ISO 14044: Environmental management — Life cycle
construction products and building elements - assessment — Requirements and guidelines
Classification using test data from reaction to fire tests
EN 14707
8 Environmental Product Declaration NMC sa – CLIMAFLEX®naturefoam exzentro
EN 14707: 2012: Thermal insulating products for
building equipment and industrial installations. Gabi ts
Determination of maximum service temperature for GaBi 10 GaBi Software-System and Database for Life
preformed pipe insulation Cycle Engineering Copyright © 1992-2021 Sphera
Solutions Gmbh Version: 10.5.0.78 DB Schema 8007
EN 15804
EN 15804: 2012-04 + A1 2014: Sustainability of Institut Bauen und Umwelt
construction works — Environmental Product Institut Bauen und Umwelt e.V., Berlin(pub.): General
Declarations — Core rules for the product category of Instructions for the EPD Programme of Institut Bauen
construction products und Umwelt e.V., Version 2.0 2021
CEN/TR 15941 Product Category Rules for Building-Related
CEN/TR 15941: Sustainability of construction works - Products and Services
Environmental product declarations - Methodology for Institute Construction and Environment e.V. (IBU)
selection and use of generic data Part A: Calculation Rules for the Life Cycle
Assessment and Requirements on the Project Report
CEN TS 16516 Version 1.7
CEN TS 16516: /AgBB/, /ISO 16000-3/, /ISO 16000-6/,
/ISO16000-9/, /ISO 16000-11/ Construction products - PCR Guidance-Texts for Building-Related Products
Assessment of release of dangerous substances. and Services
Determination of emissions into indoor air From the range of Environmental Product Declarations
of Institute Construction and Environment e.V. (IBU)
EN 16783 Part B: Requirements on the EPD for Insulating
EN 16783: 2017 Thermal insulation products - Product materials made of foam plastics
category rules (PCR) for factory made and in-situ Version 1.6 (Template) Version 1.2 (PCR specific)
formed products for preparing environmental product
declarations Sphera
Sphera Solutions Gmbh. GaBi 10 LCI documentation.
Eurostat GaBi Databases (sphera.com) Stuttgart,
European Statistics: Recovery rates for packaging Echterdingen: Sphera Solutions Gmbh
waste Paper and cardboard packaging for the
European Union 27 countries 2014
http://ec.europa.eu/eurostat/home
Eurofins
Eurofins: Product Testing Institute
9 Environmental Product Declaration NMC sa – CLIMAFLEX®naturefoam exzentro
Publisher
Institut Bauen und Umwelt e.V. Tel +49 (0)30 3087748- 0
Panoramastr. 1 Fax +49 (0)30 3087748- 29
10178 Berlin Mail info@ibu-epd.com
Germany Web www.ibu-epd.com
Programme holder
Institut Bauen und Umwelt e.V. Tel +49 (0)30 - 3087748- 0
Panoramastr 1 Fax +49 (0)30 – 3087748 - 29
10178 Berlin Mail info@ibu-epd.com
Germany Web www.ibu-epd.com
Author of the Life Cycle
Assessment Tel +32 (0) 87 85 85 00
NMC S.A. Fax +32 (0) 87 85 85 11
Gerd-Noël-Strasse 1 Mail info@nmc.eu
4731 Eynatten Web www.nmc.eu
Belgium
Owner of the Declaration
NMC S.A. Tel +32 (0) 87 85 85 00
Gerd-Noël-Strasse 1 Fax +32 (0) 87 85 85 11
4731 Eynatten Mail info@nmc.eu
Belgium Web www.nmc.eu
