ENVIRONMENTAL PRODUCT DECLARATION
as per ISO 14025 and EN 15804+A1
Owner of the Declaration Sika Deutschland CH AG & Co KG
Publisher Institut Bauen und Umwelt e.V. (IBU)
Programme holder Institut Bauen und Umwelt e.V. (IBU)
Declaration number EPD-MDS-20210038-CBA5-EN
Issue date 08.06.2021
Valid to 07.06.2026
Cement-based insulation foam: Sikatherm NFF 2070 IN
Sika Deutschland CH AG & Co KG
www.ibu-epd.com | https://epd-online.com
General Information
Sika Deutschland CH AG & Co KG Cement-based insulation foam: Sikatherm NFF
2070 IN
Programme holder Owner of the declaration
IBU – Institut Bauen und Umwelt e.V. Sika Deutschland CH AG & Co KG
Hegelplatz 1 Kornwestheimer Straße 103 - 107
10117 Berlin 70439 Stuttgart
Germany Germany
Declaration number Declared product / declared unit
EPD-MDS-20210038-CBA5-EN 1m3 cement-based insulation foam Sikatherm NFF 2070 IN, with an
average density of 76.02 kg/m3 and a dry density of 70 kg/m3.
This declaration is based on the product category rules: Scope:
cement-based foams, 19.07.2023 The ecobalance is based on the compound Sikatherm NFF 2000 IN
(PCR checked and approved by the SVR) produced by BauMineral GmbH by order of Sika Deutschland GmbH. The
board SwissPorit, Sikatherm NFF 2070 IN produced out of the compound,
is produced by Eberhard Bau AG (CH) until the end of 2021 and by the
Issue date Swiss Porit AG from the beginning of 2022. The results of the ecobalance
are mainly dominated by the compound production. Therefore, the results
08.06.2021
may serve as a good approximation for other board production locations.
The owner of the declaration shall be liable for the underlying information
and evidence; the IBU shall not be liable with respect to manufacturer
Valid to
information, life cycle assessment data and evidences.
07.06.2026
The EPD was created according to the specifications of EN 15804+A1. In
the following, the standard will be simplified as EN 15804.
Verification
The standard EN 15804 serves as the core PCR
Independent verification of the declaration and data according to ISO
14025:2011
internally X externally
Dipl.-Ing. Hans Peters
(Chairman of Institut Bauen und Umwelt e.V.)
Florian Pronold Dr. Eva Schmincke,
(Managing Director Institut Bauen und Umwelt e.V.) (Independent verifier)
1 Environmental Product Declaration - Sika Deutschland CH AG & Co KG - Cement-based insulation foam: Sikatherm NFF 2070 IN
Product
Product description/Product definition Technical Data
Under the Sika Deutschland GmbH, the Sikatherm brand
Constructional Data
combines its technological know-how and comprehensive
Name Value Unit
product portfolio to provide the right solutions, based on our
experience gained in countless construction projects worldwide. Gross density 67 - 72 kg/m3
Dimensional stability <2 %
SwissPorit / Sikatherm NFF 2070 IN boards are an inorganic
Thermal conductivity 37.5 - 38.5 W/(mK)
insulation material consisting of an inorganic binder and
Specific heat capacity 1.1 kJ/kgK
inorganic fillers. It is an easy to process material for light, non-
Water vapour diffusion resistance factor 1.5 -
flammable and thermally insulating as well as completely
recyclable products used in the construction industry. Compressive strength 25 kPa
Flexural stress 20 kPa
Sikatherm NFF 2070 IN has been specially developed for Tensile strength 9 kPa
permanent, energy-efficient and heat-insulating prefabrication
Melting point 1300 °C
and construction site applications.
Building material class A1 -
At high, medium and low densities, the product is frost-resistant Equilibrium moisture content 5 %
and shows little water absorption because it has a high Performance data of the product with respect to its
proportion of closed pores. Furthermore, it has a high level of characteristics in accordance with the relevant technical
stability when exposed to cyclical temperature and humidity. provision (no CE-marking).
The product is manufactured in a chemical foaming process Base materials/Ancillary materials
(reaction of hydrogen peroxide and a catalyst to form water and Name Value Unit
oxygen). This can be carried out continuously or in a batch
Cement 30-40 M.%
process.
Kaolin (calcinated) 15-25 M.%
For the use of the product, the respective national regulations Fly ash 15-25 M.%
at the place of use apply, in Germany for example the building Stabilizer 5-15 M.%
regulations of the federal states, and the technical regulations Gypsum 5-10 M.%
based on these regulations.
Mineral filler 0-10 M.%
Application PP-fibers 0-1 M.%
Renovation, repair and new construction Hydrophobing agent 0-0.5 M.%
• Interior insulation of ceiling, wall and roof In addition, 90-120 mass% water (based on solids) is used in
• Underside insulation ceiling / roof the production. Formwork oil is used as an auxiliary material.
• Insulation between rafters
• Core insulation Cement: Cement serves as the main binder and is made by
• Insulation of double-leaf walls burning limestone, bauxite and calcium sulfate and then mixing
• Insulation wood frame construction and grinding with gypsum.
• External insulation of the wall behind the cladding
(ventilated facade) Hard coal fly ash: Hard coal fly ash is produced when coal is
• External insulation wall behind plaster (External Thermal burned. Fly ash is involved in the development of strength
Insulation Composite Systems, ETICS) when water is added and serves as a secondary binder.
• Insulation of apartment and room partition walls
• Screed insulation Calcined kaolin: The calcined kaolin is a kaolin that is
• Brick cavity insulation (brick and concrete) homogenized by a burning process. The resulting metakaolin
The insulation panels are processed and applied by hand. The compacts the structure and participates in the development of
cutting is done using a band saw or hard metal saws. The strength.
insulation panels are attached with an adapted mortar and
plaster system. Plastic dowels can also be used. The insulation Anhydride / gypsum: the reactivity of the cement is controlled
boards can be plastered, painted or coated. by adding anhydride.
Formwork oil: An oil based on renewable raw materials is used
as formwork oil and is easily biodegradable. Formwork oil is
used as a release agent.
Water-repellent agent: The water-repellent agent is used to
reduce water absorption. Metal soaps that are partially
hydrophilic and hydrophobic are used.
Mineral surcharge: The surcharge comes from ground
production residues of the insulation boards themselves.
PP fibres: The use of extruded PP fibres significantly increases
flexural strength and adhesive strength.
2 Environmental Product Declaration - Sika Deutschland CH AG & Co KG - Cement-based insulation foam: Sikatherm NFF 2070 IN
Air stabilizers: Fine-grained inorganic carbonates are used for
air stabilization, which have been functionalized beforehand. Reference service life
The partially hydrophobized particles form a boundary layer When used as intended, the service life of the insulation boards
between the air and water phases. is <50 years according to the Bundesinstitut für Bau-, Stadt-
und Raumforschung (BBSR) table 'Service life of components
This product contains substances listed in the candidate list for life cycle analyzes according to the assessment system for
( 01.05.2020) exceeding 0.1 percentage by mass: no sustainable building (BNB)'.
LCA: Calculation rules
multiplied with the respective loss rate.
Declared Unit
The declared unit is 1 m³ of Sikatherm NFF 2070 IN foam with Module B1:
an average density at factory gate of 76,02 kg/m³. Carbonation of Ettringite (55% carbonation rate; 95%
Declared Unit carbonation rate in total).
Name Value Unit
Module C1:
Declared unit 1 m3 Manual deconstruction (no loads).
Gross density (wet) 76.02 kg/m3
Gross density (abs. dry) 65 kg/m³ Module C2:
Transport to the waste treatment plant (50 km by truck).
Conversion factor to 1 kg 76,02 kg/m³
Transport distance may be adjusted on building level if relevant.
Other declared units are allowed if the conversion is shown
transparently. Module C3/1:
Recycling as admixture in cement foam production. Average
efforts for waste treatment (shredding).
System boundary
Type of the EPD: cradle to gate - with options.
Module C3/2:
Recycling as backfill material. Average efforts for waste
Module A1:
treatment (shredding).
Raw material and energy supply for production of the
(foamable) compound. Packaging materials.
Module D/1:
Avoided burdens for substitution of kaolin and calcium
Module A2:
carbonate (non-reactive compound constituents).
Transport of the compound to the converter Switzerland.
Module D/2:
Module A3:
Avoided burdens for substitution of gravel.
Foaming, forming and cutting of the compound. Treatment of
compound packaging. Foam curing incl. carbonation Geographic Representativeness
(carbonation rate of 40% within A3, which leads to a carbon Land or region, in which the declared product system is
uptake of 1.04 kg CO 2). Packaging of foam. manufactured, used or handled at the end of the product´s
lifespan: Europe
Module A4:
Transport to the construction site (100 km by truck). Trnasport
Comparability
distance may be adjusted on building level if relevant.
Basically, a comparison or an evaluation of EPD data is only
Module A5: possible if all the data sets to be compared were created
Packaging treatment. Installation losses have not been according to EN 15804 and the building context, respectively
accounted for since these highly depend on the building context the product-specific characteristics of performance, are taken
and application. Eventual losses may be estimated using the into account.
indicator results for the manufacturing phase (modules A1-A3)
LCA: Scenarios and additional technical information
Reference service life
Name Value Unit
Transport from the gate to the site (A4)
Life Span (according to BBSR) 50 a
Name Value Unit
Litres of fuel 136 l/100km End of Life (C1-C4)
Transport distance 100 km Name Value Unit
Capacity utilisation (including empty runs) 61 % Collected separately waste type type 1 kg
Gross density of products transported 76.02 kg/m3 Collected as mixed construction waste - kg
Reuse - kg
Use or application of the installed product (B1) see section
Recycling 0.97 kg
2.12 "Use"
Energy recovery - kg
Name Value Unit
Landfilling 0.03 kg
Carbonatization rate in the use phase 55 %
Carbon uptake in the use phase 1,46 kg CO2
3 Environmental Product Declaration - Sika Deutschland CH AG & Co KG - Cement-based insulation foam: Sikatherm NFF 2070 IN
LCA: Results
DESCRIPTION OF THE SYSTEM BOUNDARY (X = INCLUDED IN LCA; MND = MODULE NOT DECLARED; MNR = MODULE NOT
RELEVANT)
Benefits and
Construction loads beyond
Product stage Use stage End of life stage
process stage the system
boundaries
la ire ta m w a Ry lp p u s tro p s n a rT g n iru tc a fu n a M e h t m o rf tro p s n a rTe tis e h t o t e ta g y lb m e s s A e s U e c n a n e tn ia M ria p e R tn e m e c a lp e R tn e m h s ib ru fe R y g re n e la n o ita re p Oe s u re ta w la n o ita re p Oe s u n o itc u rts n o c -e Dn o itilo m e d tro p s n a rT g n is s e c o rp e ts a W la s o p s iD -e s u e R-y re v o c e R-g n ilc y c e Rla itn e to p
A1 A2 A3 A4 A5 B1 B2 B3 B4 B5 B6 B7 C1 C2 C3 C4 D
X X X X X X MND MNR MNR MNR MND MND MND X X MND X
RESULTS OF THE LCA - ENVIRONMENTAL IMPACT according to EN 15804+A1: 1 m³ cement-based insulation foam
Parameter Unit A1-A3 A4 A5 B1 C2 C3/1 C3/2 D/1 D/2
GWP kg CO 2 eq 45.59 0.478 7.62 -1.46 0.447 0.164 0.164 -32.39 -2.718
ODP kg CFC11 eq 1.05E-06 7.82E-17 1.08E-15 0 7.31E-17 5.46E-16 5.46E-16 -2.32E-13 -3.87E-14
AP kg SO 2 eq 1.09E-01 3.73E-04 6.42E-04 0 3.49E-04 1.15E-03 1.15E-03 -2.69E-02 -3.64E-03
EP kg PO 43 eq 3.5E-02 6.86E-05 1.39E-04 0 6.42E-05 2.76E-04 2.76E-04 -4.86E-03 -5.29E-04
POCP kg Ethen eq 6.96E-03 -1.61E-06 5.67E-05 0 -1.5E-06 1.27E-04 1.27E-04 -3.04E-03 -3.64E-04
ADPE kg Sb eq 7.35E-05 3.5E-08 1.33E-08 0 3.28E-08 1.85E-07 1.85E-07 -3.75E-06 -4.82E-07
ADPF MJ 660.7 6.48 1.21 0 6.06 3.19 3.19 -495.5 -38.16
GWP = Global warming potential; ODP = Depletion potential of the stratospheric ozone layer; AP = Acidification potential of land and water; EP =
Eutrophication potential; POCP = Formation potential of tropospheric ozone photochemical oxidants; ADPE = Abiotic depletion potential for non-fossil
resources; ADPF = Abiotic depletion potential for fossil resources
RESULTS OF THE LCA - INDICATORS TO DESCRIBE RESOURCE USE according to EN 15804+A1: 1 m³ cement-based
insulation foam
Parameter Unit A1-A3 A4 A5 B1 C2 C3/1 C3/2 D/1 D/2
PERE MJ 133.17 0.365 52.5 0 0.342 0.238 0.238 -44.88 -10.378
PERM MJ 52.19 0 -52.2 0 0 0 0 0 0
PERT MJ 185.47 0.365 0.265 0 0.342 0.238 0.238 -44.88 -10.378
PENRE MJ 657.8 6.5 33.7 0 6.08 14.1 14.1 -517 -46.99
PENRM MJ 43.1 0 -32.3 0 0 -10.8 -10.8 0 0
PENRT MJ 700.8 6.5 1.42 0 6.08 3.3 3.3 -517 -46.99
SM kg 13 0 0 0 0 0 0 0 0
RSF MJ 0 0 0 0 0 0 0 0 0
NRSF MJ 0 0 0 0 0 0 0 0 0
FW m3 1.72E-01 4.23E-04 1.79E-02 0 3.95E-04 9.29E-04 9.29E-04 -3.26E-02 -1.2E-02
PERE = Use of renewable primary energy excluding renewable primary energy resources used as raw materials; PERM = Use of renewable primary
energy resources used as raw materials; PERT = Total use of renewable primary energy resources; PENRE = Use of non-renewable primary energy
excluding non-renewable primary energy resources used as raw materials; PENRM = Use of non-renewable primary energy resources used as raw
materials; PENRT = Total use of non-renewable primary energy resources; SM = Use of secondary material; RSF = Use of renewable secondary fuels;
NRSF = Use of non-renewable secondary fuels; FW = Use of net fresh water
RESULTS OF THE LCA – WASTE CATEGORIES AND OUTPUT FLOWS according to EN 15804+A1:
1 m³ cement-based insulation foam
Parameter Unit A1-A3 A4 A5 B1 C2 C3/1 C3/2 D/1 D/2
HWD kg 5.85E-04 3.03E-07 9.82E-10 0 2.83E-07 8.64E-08 8.64E-08 -3.63E-07 -5.42E-08
NHWD kg 1.05E+00 9.95E-04 4.69E-02 0 9.31E-04 8.92E-04 8.92E-04 -1.46E+00 -2.65E+00
RWD kg 5.7E-03 8.05E-06 8.15E-05 0 7.53E-06 4.36E-05 4.36E-05 -8.38E-03 -3.5E-03
CRU kg 0 0 0 0 0 0 0 0 0
MFR kg 0 0 0 0 0 63 63 0 0
MER kg 0 0 0 0 0 0 0 0 0
EEE MJ 0 0 11.3 0 0 0 0 0 0
EET MJ 0 0 20.2 0 0 0 0 0 0
HWD = Hazardous waste disposed; NHWD = Non-hazardous waste disposed; RWD = Radioactive waste disposed; CRU = Components for re-use;
MFR = Materials for recycling; MER = Materials for energy recovery; EEE = Exported electrical energy; EET = Exported thermal energy
4 Environmental Product Declaration - Sika Deutschland CH AG & Co KG - Cement-based insulation foam: Sikatherm NFF 2070 IN
References
Standards Further References
EN 15804/A1 BBSR - Bundesinstitut für Bau-, Stadt- und
EN 15804:2012-04+A1 2013, Sustainability of construction Raumforschung
works — Environmental Product Declarations — Core rules for Service Life of Building Components; version 24.02.2017.
the product category of construction products. https://www.nachhaltigesbauen.de/fileadmin/pdf/Nutzungsdauer
_Bauteile/BNB_Nutzungsdauern_von_Bauteilen_2017-02-
ISO 14025 24.pdf
DIN EN ISO 14025:2011-10, Environmental labels and
declarations — Type III environmental declarations — GaBi
Principles and procedures. GaBi Software version 9.5.1, Sphera Solutions GmbH,
Stuttgart. GaBi Professional database, Service Pack 40, 2020.
IBU 2016
Institut Bauen und Umwelt e.V.: General Programme
Instructions for the Preparation of EPDs at the Institut Bauen
und Umwelt e.V. Version 1., Berlin: Institut Bauen und Umwelt
e.V., 2016. "http://www.ibu-epd." www.ibu-epd.com
PCR Product Category Rules for Building-Related Products
and Services
Institut Bauen und Umwelt e.V.: PCR part A: Calculation Rules
for the life Cycle Assessment and Requirements on the Project
Report, v1.8, 2019.
Institut Bauen und Umwelt e.V.: PCR part B: Requirements on
the EPD for cement-based foams, 2020.
5 Environmental Product Declaration - Sika Deutschland CH AG & Co KG - Cement-based insulation foam: Sikatherm NFF 2070 IN
Publisher
Institut Bauen und Umwelt e.V. +49 (0)30 3087748- 0
Hegelplatz 1 info@ibu-epd.com
10117 Berlin www.ibu-epd.com
Germany
Programme holder
Institut Bauen und Umwelt e.V. +49 (0)30 3087748- 0
Hegelplatz 1 info@ibu-epd.com
10117 Berlin www.ibu-epd.com
Germany
Author of the Life Cycle Assessment
Sphera Solutions GmbH +49 711 341817-0
Hauptstraße 111- 113 info@sphera.com
70771 Leinfelden-Echterdingen www.sphera.com
Germany
Owner of the Declaration
Sika Deutschland CH AG & Co KG +49 (0)711 80 09-0
Kornwestheimer Straße 103 - 107 info@de.sika.com
70439 Stuttgart www.sika.de
Germany
6 Environmental Product Declaration - Sika Deutschland CH AG & Co KG - Cement-based insulation foam: Sikatherm NFF 2070 IN
