ENVIRONMENTAL-PRODUCT DECLARATION
as per ISO 14025 and EN 15804+A2
Owner of the Declaration Hilti Aktiengesellschaft
Publisher Institut Bauen und Umwelt e.V. (IBU)
Programme holder Institut Bauen und Umwelt e.V. (IBU)
Declaration number EPD-HIL-20220306-IBA1-EN
Issue date 31/01/2023
Valid to 30/01/2028
HIT-HY 170
Hilti AG
www.ibu-epd.com | https://epd-online.com
1. General Information
Hilti AG HIT-HY 170
Programme holder Owner of the declaration
IBU – Institut Bauen und Umwelt e.V. Hilti Aktiengesellschaft
Hegelplatz 1 Feldkircher Strasse 100
10117 Berlin 9494 Schaan
Germany Liechtenstein
Declaration number Declared product / declared unit
EPD-HIL-20220306-IBA1-EN The
declared product is a HILTI injectable mortar HIT-HY 170. The declared
unit
is one kilogram of reaction resin product in the mixing ratio of the two
components necessary for processing. The packaging is also included in
the
calculation. The declared unit is stated in [kg].
This declaration is based on the product category rules: Scope:
Reaction resin products, 01/08/2021 This
(PCR checked and approved by the SVR) document refers to the injectable mortar HIT-HY 170 with its packaging.
For
the compilation of the life cycle assessment, specific data were collected
Issue date from
the factory in Kaufering, Germany, of the HILTI AG. For the compilation of
31/01/2023
the life cycle assessment, specific data were collected from the factory in
Kaufering, Germany, of the HILTI AG. Data from the years 2018 to 2021
are used, which correspond to the annual average.
Valid to
The owner of the declaration shall be liable for the underlying information
30/01/2028 and evidence; the IBU shall not be liable with respect to manufacturer
information, life cycle assessment data and evidences.
The EPD was created according to the specifications of EN 15804+A2. In
the following, the standard will be simplified as EN 15804 bezeichnet.
Verification
The standard EN 15804 serves as the core PCR
Independent verification of the declaration and data according to ISO
14025:2011
internally X externally
Dipl.-Ing Hans Peters
(chairman of Institut Bauen und Umwelt e.V.)
Dr. Alexander Röder Matthias Klingler,
(Managing Director Institut Bauen und Umwelt e.V.) (Independent verifier)
1 Environmental-Product Declaration - Hilti AG - HIT-HY 170
2. Product
2.1 Product description/Product definition ETA 15/0197
The declared product of HIT-HY 170 is a
two component system. The resin component (component A)
comprises a resin based
on methacrylate as well as mineral and cementitious fillers. The ETA 14/0457
curing agent component (component B) comprises peroxide
hardener, water and
mineral fillers. Mixing the two components A and B in the static
mixer and the CE marking. For the
initiates the curing (hardening) reaction of both binder systems. application and use the respective national provisions apply.
During the
curing phase, a very strong bond is formed between the 2.2 Application
organic and inorganic Hilti
binder matrix. The hybrid system formed during cement and HIT-HY
resin curing results 170 serves for safely securing threaded rods and post-installed
in a crosslinked duromer with desired design properties (high rebar
bond strengths connections in cracked and uncracked concrete C20/25 to
within a short curing time) and particular durability. C50/60. HIT-HY170 is ETA
Composite foils are used for the two component foil pack of approved for seismic C2 category for anchoring. Hilti HIT-
HIT-HY170. This HY170 is a
kind of packaging serves the following purposes: waste volume component of the Hilti SAFEset concept. Hilti SAFEset is an
reduction, easy approved system
storage and transport, and less packaging material. which makes anchor installation an easier, safer and faster
process. It
significantly improves the robustness of fastening and
dramatically reduces the
Through legislation and possibilities of error during installation. As part of SAFEset HIT-
increased public awareness users have increasingly become HY170 can be
discerned towards the installed with approved Hilti Hollow Drill bits and vacuum
use of styrene and other highly volatile components with their cleaners that drill
resulting and clean the hole in one step for virtually dust-free installation.
unpleasant odour and low flash point (flammability). The use of
Hilti HDE22 dispenser with the Volume Calculator App leads to
no under or over
The reaction resins fill, reducing underfilling related risks and minimizing mortar
used in all Hilti hybrid adhesives contain no styrene, are wastage.
practically odourless
and have a considerably higher flash point, i.e. higher than 2.3 Technical Data
100°C in The technical specifications of the products within the scope of
comparison to 34° C for styrene based products. HIT-HY170 is the EPD shall be listed, including the reference to the test
a methods/test standards for each specification.
premium performance injectable hybrid mortar with approvals
for rebar For products with CE marking, the technical specifications must
connections and heavy-duty anchoring. For the placing of the be specified in accordance with information in the declaration of
product performance. The properties relevant to the product should be
on the market in the European Union European Free Trade specified in the table below. If no information is given for
Association EU/EFTA) properties, an explanation must be given in the background
(with the exception of Switzerland) the Regulation (EU) No. report to the EPD as to why the property is not relevant to the
305/2011 (CPR) product.
applies. The product needs a declaration of performance taking
into Constructional data
consideration the following European Technical Approvals
Name Value Unit
Density acc. to ISO 2811-1 1710 kg/m3
Compressive strength (20°C) acc. to EN ISO 604 79 N/mm2
ETA 19/0465 Elastic modulus (pressure) acc. to EN ISO 604 2096 N/mm2
Tensile strength (20°C) acc. to EN ISO 527-1;
14,4 N/mm2
type 1A - EN ISO 527-2
Tensile modulus acc. to EN ISO 527-1; type 1A -
ETA 19/0161 3697 N/mm2
EN ISO 527-2
Hilti HIT-HY 170 displays the
following characteristics:
ETA 15/0297
2 Environmental-Product Declaration - Hilti AG - HIT-HY 170
Performance data of the
product in accordance with the declaration of performance with
respect to its
essential characteristics according to > 10°C
to +20 °C 5 min
ETA 19/0465
> 20°C
to +30 °C 3 min
ETA 19/0161
> 30°C
to +40 °C 2 min
ETA 15/0297
ETA 15/0197
Curing time:
ETA 14/0457
-5°C to 0 °C 12 hours
> 0°C to 5 °C 5 hours
Shelf life:
> 5°C to +10 °C 2.5 hours
12 months
> 10°C to
+20 °C 1.5 hours
Substrate temperature during > 20°C
installation: to +30 °C 45 min
> 30°C
-5°C to +40 °C to +40 °C 30 min
2.4 Delivery status
The product Hilti HIT-HY 170 is available in foil-packages with a
total of 330 ml and 500 ml injectable mortar in the
corresponding mixing ratio.
2.5 Base materials/Ancillary materials
Working time: Hilti HIT-HY 170 is supplied in the form of a dual component
film-wrapped pack comprising a resin component and a curing
agent component at a volume ratio of 3:1. The mixing ratio of
resin and curing agent components is automatically set during
-5°C the injection process. Product curing commences directly after
to 0 °C 10 min the components are mixed.
The product reviewed in this EPD contains the following
component volumes:
> 0°C to 5 °C 10 min
Resin component:
Methacrylate resin mixture: 40 to 50 % by weight
Mineral fillers: 30 to 40 % by weight
> 5°C to +10 °C 8 min Cement: 10 to 20 % by weight
3 Environmental-Product Declaration - Hilti AG - HIT-HY 170
Other: < 5 % by weight 4) Put the cassette into the dispenser system
5) Discard the first trigger pulls
Curing agent component: 6) Fill 2/3 of the borehole with mortar
Mineral fillers: 50 to 60 % by weight 7) Set the fixing element
Water: 20 to 30 % by weight After mixing the components and squeezing the mortar into the
Dibenzoyl peroxide: 5 to 10 % by weight borehole the fixing element has to be set within the working
Other: < 6 % by weight time mentioned in the Instructions for Use. After the curing time,
described as well in the Instructions for Use, the mortar is ready
This product article contains substances listed in the candidate to take up loads.
list (date: 30.06.2022) exceeding 0.1 percentage by mass: no.
2.9 Packaging
This product contains other Carcinogenic, Mutagenic, Hilti HIT-HY 170 is supplied in the form of a 2-foil-pack system
Reprotoxic (CMR) substances in categories 1A or 1B which are and thus leads to very little waste remaining after use on the
not on the candidate list, exceeding 0.1 percentage by mass: construction site. After curing, the product can be disposed of
no. with household waste. Full or only partially emptied cartridges
must be disposed of as special waste in accordance with official
Biocide products were added to this construction product or it regulations.
has been treated with biocide products (this then concerns a The outer packaging consisting of plastic foil and cardboard
treated product as defined by the (EU) Ordinance on Biocide boxes designed according to the product size can be recycled.
Products No. 528/2012): no. Packaging contaminated by the product must be disposed in a
safe manner in
2.6 Manufacture accordance with local/national regulations.
Most raw materials are sourced in Europe. The transport is
exclusively by truck for the European raw materials, and by 2.10 Condition of use
truck and by ship for the others. During
Chemical mortars are usually two-component systems the installation the temperature of the base material must be
consisting of a binder and a hardener. One of the base between -5°C and
components of the binder is the reactive resin which in the case +40°C when used in concrete or hollow bricks and +5°C and
of HIT-HY 170 is produced in Kaufering. +40°C when used in solid
The resin production process is a chemical reaction of the clay bricks. The temperature of the product should be between
corresponding educts to a basic resin with subsequent mixing +5°C to +25°C during storage and +5°C to +40°C during usage.
of the basic resin with different reactive diluents to a reactive Hilti literature and
resin. This process is controlled and monitored by process official approvals must always be considered. The two
control components of HIT-HY 170 are
technology. only for use in combination with the defined volume ratio and
The production of chemical mortars consists of a mixing under the
process and a filling process of the respective single conditions mentioned above to build up a crosslinked filled
components (binder and hardener) and their subsequent union duromer.
to a two-component system (packaging). Here as well process
2.11 Environment and health during use
control technology is used to weigh and mix solid and liquid
compounds according to the specification. In the next step both Refer to the Safety Data Sheet (SDS) for detailed information
well-mixed components run through an automized filling line in on handling, storage as well as first aid, firefighting and
which each of the processed masses is filled into a tubular foil accidental release measures and disposal considerations.
bag. Finally the single components are combined in one Following the given
packaging unit. The two-pack foil bags are packed into instructions help to minimize the risk to health and environment.
cardboard boxes and then finally shipped.
2.12 Reference service life
The manufacturing plant of HIT-HY 170, Hilti GmbH
Hilti HIT-HY 170 is exposed to a wide variety of environmental
Industriegesellschaft für Befestigungstechnik, Hiltistr. 6, 86916
factors during the use phase. The anticipated Reference
Kaufering, Germany, is certified according to ISO 9001. The
Service Life depends on the specific installation situation and
guideline defines international standards for quality and
the product exposure scenario. The main factors influencing the
process management.
period of use involve weathering as well as mechanical loads
2.7 Environment and health during manufacturing and chemical exposure.
The manufacturing plant of HIT-HY 170,Hilti GmbH Description of the influences on the ageing of the product when
Industriegesellschaft für Befestigungstechnik, Hiltistr. 6, 86916 applied in accordance with the rules of technology.
Kaufering, Germany, is certified according to ISO 14001 which
defines international standards for sustainable environmental
2.13 Extraordinary effects
management.
Fire
The production site is also certified in accordance with ISO
Even
50001 Energy Management Systems.
without any special fire safety features the Injection Systems
2.8 Product processing/Installation comply with at
least the requirements of the DIN EN 13501-1 standard for fire
The product is delivered with Instructions for Use explaining the
classes E and
basic steps for installation:
Efl. As crosslinked methacrylate resins do not melt or drip, the
1) For safe handling the precautionary measures
resins do not
described in the Safety Data Shhet (SDS) (e.g. hand and eye
contribute towards spreading fire. Apart from the common
protection)
combustion produces
must be adhered to
carbon monoxide and carbon dioxide, fire gases can contain
2) Insert the cartridge into the black cassette
traces of methyl
3) Screw on the mixing nozzle
4 Environmental-Product Declaration - Hilti AG - HIT-HY 170
methacrylate, esters, alcohol, and hydrocarbons. Due to the
quantities used, Mechanical destruction
they only have a subordinate influence on the fire It
characteristics of a is recommended to use dust protection during the demolition of
building structure in which they have been installed. the cured chemical
anchor.
Fire protection
Name Value 2.14 Re-use phase
Building material class E/Efl The product cannot be reused. After usage the product can be
Burning droplets No performance assessed removed by demolition.
Smoke gas development No performance assessed
2.15 Disposal
Uncured Hilti HIT-HY 170 can be disposed of according to the
Water European waste code 08 04 09* or 20 01 27*. The built-in cured
The anchor can be disposed as construction waste for which the
cured product is chemically inert and insoluble in water. HIT-HY European waste code 17 01 01 applies.
170 is
certified for use as an anchoring adhesive in concrete for water 2.16 Further information
treatment Further information is available on request under
applications according to National Sanitation Foundation (US) anchor.hse@hilti.com and on the Hilti website:
NSF. www.hilti.group
3. LCA: Calculation rules
3.1 Declared Unit
The product declared here is an injection mortar from HILTI AG
with the designation HIT-HY 170. The declared unit refers to 1
kg reaction resin product in the mixing ratio of the two End of life
components required for processing. The packaging, based on (C1- C4):
1 kg of reaction resin product, is also calculated at 0.149 kg.
The table below shows the data of the declared unit.
Declared unit
• C1,
Name Value Unit
dismantling/demolition,
Declared unit 1 kg
For IBU core EPDs (where clause 3.6 is part of the EPD): for
average EPDs, an estimate of the robustness of the LCA
values must be made, e.g. concerning variability of the • C2,
production process, geographical representativeness and the transportation,
influence of background data and preliminary products
compared to the environmental impacts caused by actual
production.
• C3, waste
treatment,
3.2 System boundary
Type of EPD:
cradle to gate with options.The following information modules
are defined as • C4, elimination.
system boundaries in this study:
Production stage (A1- A3):
• A1, raw
material extraction, Reuse, recovery
and recycling potential (D)
• A2, transport
to manufacturer, In order to
precisely record the indicators and environmental impacts of
the declared unit,
a total of 8 information modules are considered. The
• A3, information modules A1 to
manufacture. A3 describe the provision of materials, the transport to the
production site
and the production processes of the product itself.
5 Environmental-Product Declaration - Hilti AG - HIT-HY 170
Illustration 3:
Information module A1 to A3 of packaging
3.3 Estimates and assumptions
The electricity mixes and other background data are calculated
on a country-specific basis for the production processes. For
The main products are sourced from the European Union and 1,1'-(p-tolylimino)dipropan-2-ol and 1,2-dihydroxybenzene, an
Asia. Transport is by truck and ship. The following flow charts assumption was made for the calculation of the material supply.
illustrate the underlying production process. This assumption is based on manufacturer data. No
assumptions or limitations were made for other formulation
contents or processes.
3.4 Cut-off criteria
All energy and mass inputs were taken into account.The cut-off
criterion according to EN 15804 is not applied.
3.5 Background data
The database of
the background data of the GaBi 10 and ecoinvent 3.8
databases, to which this study also refers,
is documented under the following link. (Sphera).
3.6 Data quality
For the
compilation of the life cycle assessment,
specific data
Illustration 1:
were collected from the factory Kaufering,
Information module A1 to A3 of product (part 1)
in Germany, of
the HILTI AG from the year 2022. The
background data
from the /GaBi 10 database/ used is
from the year
2022 and thus of high relevance.
The mass of the different components of the reactive
Illustration 2: resin mixture come from the information to the recipe. The data
Information module A1 to A3 of product (part 2) quality is
classified as appropriate.
3.7 Period under review
Data from 2022 is used as production has only
just started.
3.8 Geographic Representativeness
Land or region, in which the declared product system is
manufactured, used or handled at the end of the product´s
lifespan: Germany
3.9 Allocation
Allocation of co-products takes place in the
information
modules A1-A3.
The production waste of the injection-moulded
components is thermally recovered. The electrical and
6 Environmental-Product Declaration - Hilti AG - HIT-HY 170
Basically, a comparison or an evaluation of EPD data is only
thermal energy credits resulting therefrom are possible if all the data sets to be compared were created
according to EN 15804 and the building context, respectively
completely charged in modules A1-A3. the product-specific characteristics of performance, are taken
No further allocations are made. into account.
The used background database has to be mentioned.
3.10 Comparability
4. LCA: Scenarios and additional technical information
Characteristic product properties
Information on biogenic carbon In case a reference service life according to applicable ISO
standards is declared then the assumptions and in-use
No renewable conditions underlying the determined RSL shall be declared. In
raw materials are used in the product. Therefore, the biogenic addition, it shall be stated that the RSL applies for the reference
carbon is shown conditions only.
as zero. The following raw materials contain biogenic carbon in
the packaging. The same holds for a service life declared by the manufacturer.
Corresponding information related to in-use conditions needs
Information on describing the biogenic Carbon Content at
not be provided if a service life taken from the list on service life
factury gate
by BNB is declared.
Name Value Unit
Packaging Cardboard Box 0,013 kg C
End of life (C1-C4)
Packaging IfU-Lables, Paper 0,014 kg C
The
product is demolished using an electric chisel. The electrical
The following technical scenario information is required for the energy
declared modules and optional for non-declared modules. consumption for the tool is assumed to be 0.05 MJ for the
Modules for which no information is declared can be deleted; declared unit. The
additional information can also be listed if necessary. electricity consumption is calculated with a European electricity
mix. The
The following technical information is a basis for the declared construction waste is transported by truck 50 km to the waste
modules or can be used for developing specific scenarios in the treatment plant.
context of a building assessment if modules are not declared The construction waste is shredded in the waste treatment
(MND). plant and then
dumped.
A5 is not declared including the disposal of the packaging
Name Value Unit
material on the construction site, the amounts of packaging
Collected as mixed construction waste 1 kg
materials included in the LCA calculations must be declared as
technical scenario information for Module A5. Crushing in the shredder 1 kg
Landfilling 1 kg
Reuse, recovery and/or recycling potentials (D), relevant
Information on packaging
scenario information
Name Value Unit
In this calculation there are no reuse, recovery and
Componsite foil PE/PET (foil bags) 0,0089 kg recycling potentials. Therefore, the information module D is
Clips, Aluminium 0,0030 kg declared and shown
Connector, PBT 0,0204 kg as zero.
Composite foil, PE-LD 0,0092 kg Name Value Unit
Mixer, PP 0,0390 kg Reuse, recovery and recycling potentials 0 kg
Mixer extension, PE-LD 0,0050 kg
IfU- Labels, Paper 0,0333 kg
Cardboard box 0,0301 kg
7 Environmental-Product Declaration - Hilti AG - HIT-HY 170
5. LCA: Results
In Table 1 "Description of the system boundary", all declared modules shall be indicated with an "X"; all modules that are not declared
shall be indicated with "MND" (As default the modules B3, B4, B5 are marked as MNR – module not relevant). In the following tables,
columns can be deleted for modules that are not declared. Indicator values should be declared with three valid digits (eventually using
exponential form (e.g. 1,23E-5 = 0,0000123). A uniform format should be used for all values of one indicator.
If several modules are not declared and therefore have been deleted from the table, the abbreviations for the indicators can be
replaced by the complete names, while the readability and clear arrangement should be maintained; the legends can then be deleted.
If due to relevant data gaps, an indicator cannot be declared in a robust way, then the abbreviation “IND” (indicator not declared)
should be used for this indicator.
• 0 - calculated value is 0
• 0 - value falls under the cut-off
• 0 - assumption which exclude any flows (e.g. exported
electricity A1-A3)
• IND – in cases where the inventory does not support
the methodological approach or the calculation of the
specific indicator IND shall be used.
If no reference service life is declared (see chapter 2.13 "Reference Service Life"), the LCA results of the modules B1-B2 and B6-B7
shall refer to a period of one year. This shall then be indicated as an explanatory text below the tables. In addition, the formula for the
quantification of such B-modules over the total life cycle shall be provided.
DESCRIPTION OF THE SYSTEM BOUNDARY (X = INCLUDED IN LCA; ND = MODULE OR INDICATOR NOT DECLARED; MNR =
MODULE NOT RELEVANT)
BENEFITS
AND LOADS
CONSTRUCTION
BEYOND
PRODUCT STAGE PROCESS USE STAGE END OF LIFE STAGE
THE SYSTEM
STAGE
BOUNDARIE
S
la ire ta m w a Ry lp p u s tro p s n a rT g n iru tc a fu n a M e h t m o rf tro p s n a rTe tis e h t o t e ta g y lb m e s s A e s U e c n a n e tn ia M ria p e R tn e m e c a lp e R tn e m h s ib ru fe R y g re n e la n o ita re p Oe s u re ta w la n o ita re p Oe s u n o itc u rts n o c -e Dn o itilo m e d tro p s n a rT g n is s e c o rp e ts a W la s o p s iD -e s u e R-y re v o c e R-g n ilc y c e Rla itn e to p
A1 A2 A3 A4 A5 B1 B2 B3 B4 B5 B6 B7 C1 C2 C3 C4 D
X X X MND MND MND MND MNR MNR MNR MND MND X X X X X
RESULTS OF THE LCA - ENVIRONMENTAL IMPACT according to EN 15804+A2: 1 kg HILTI HIT-HY 170
Parameter Unit A1-A3 C1 C2 C3 C4 D
Global Warming Potential total (GWP-total) kg CO 2 eq 2.32E+00 5.12E-03 3.76E-03 2.6E-03 1.45E-02 0
Global Warming Potential fossil fuels (GWP-fossil) kg CO 2 eq 2.32E+00 5.12E-03 3.74E-03 2.59E-03 1.45E-02 0
Global Warming Potential biogenic (GWP-biogenic) kg CO 2 eq 0 0 0 0 0 0
Global Warming Potential luluc (GWP-luluc) kg CO 2 eq 9.14E-04 1.08E-06 2.07E-05 1.2E-05 2.67E-05 0
Depletion potential of the stratospheric ozone layer (ODP) kg CFC11 eq 2.19E-08 7.5E-14 2.22E-16 3.85E-15 3.4E-14 0
Acidification potential of land and water (AP) mol H+ eq 5.42E-03 1.12E-05 1.17E-05 1.34E-05 1.03E-04 0
Eutrophication potential aquatic freshwater (EP-freshwater) kg P eq 7.94E-05 1.49E-08 1.11E-08 7.43E-09 2.45E-08 0
Eutrophication potential aquatic marine (EP-marine) kg N eq 1.46E-03 2.52E-06 5.37E-06 6.11E-06 2.62E-05 0
Eutrophication potential terrestrial (EP-terrestrial) mol N eq 1.57E-02 2.65E-05 6.01E-05 6.74E-05 2.88E-04 0
Formation potential of tropospheric ozone photochemical oxidants kg NMVOC
4.37E-03 6.82E-06 1.05E-05 1.66E-05 7.97E-05 0
(POCP) eq
Abiotic depletion potential for non fossil resources (ADPE) kg Sb eq 4.07E-06 1.4E-09 3.1E-10 2.87E-09 1.48E-09 0
Abiotic depletion potential for fossil resources (ADPF) MJ 4.72E+01 9.29E-02 4.96E-02 5.06E-02 1.9E-01 0
m3 world eq
Water use (WDP) 2.14E-01 1.17E-03 3.33E-05 4.99E-04 1.59E-03 0
deprived
RESULTS OF THE LCA - INDICATORS TO DESCRIBE RESOURCE USE according to EN 15804+A2: 1 kg HILTI HIT-HY 170
Parameter Unit A1-A3 C1 C2 C3 C4 D
Renewable primary energy as energy carrier (PERE) MJ 5.86E+00 5.16E-02 2.82E-03 4.06E-03 2.85E-02 0
Renewable primary energy resources as material utilization
MJ 9.5E-01 0 0 0 0 0
(PERM)
Total use of renewable primary energy resources (PERT) MJ 6.81E+00 5.16E-02 2.82E-03 4.06E-03 2.85E-02 0
Non renewable primary energy as energy carrier (PENRE) MJ 4.37E+01 9.3E-02 4.97E-02 5.07E-02 1.9E-01 0
Non renewable primary energy as material utilization (PENRM) MJ 3.59E+00 0 0 0 0 0
Total use of non renewable primary energy resources (PENRT) MJ 4.73E+01 9.3E-02 4.97E-02 5.07E-02 1.9E-01 0
Use of secondary material (SM) kg 6.97E-02 0 0 0 0 0
Use of renewable secondary fuels (RSF) MJ 0 0 0 0 0 0
Use of non renewable secondary fuels (NRSF) MJ 0 0 0 0 0 0
8 Environmental-Product Declaration - Hilti AG - HIT-HY 170
Use of net fresh water (FW) m3 9.71E-03 4.92E-05 3.19E-06 1.42E-05 4.82E-05 0
RESULTS OF THE LCA – WASTE CATEGORIES AND OUTPUT FLOWS according to EN 15804+A2:
1 kg HILTI HIT-HY 170
Parameter Unit A1-A3 C1 C2 C3 C4 D
Hazardous waste disposed (HWD) kg 2.38E-08 8.04E-12 2.38E-13 6.34E-13 9.75E-12 0
Non hazardous waste disposed (NHWD) kg 5.03E-02 7E-05 7.13E-06 1.34E-05 9.71E-01 0
Radioactive waste disposed (RWD) kg 7.24E-04 1.49E-05 6.13E-08 6.68E-07 2.11E-06 0
Components for re-use (CRU) kg 0 0 0 0 0 0
Materials for recycling (MFR) kg 0 0 0 0 0 0
Materials for energy recovery (MER) kg 0 0 0 0 0 0
Exported electrical energy (EEE) MJ 0 0 0 0 0 0
Exported thermal energy (EET) MJ 0 0 0 0 0 0
RESULTS OF THE LCA – additional impact categories according to EN 15804+A2-optional:
1 kg HILTI HIT-HY 170
Parameter Unit A1-A3 C1 C2 C3 C4 D
Disease
Incidence of disease due to PM emissions (PM) ND ND ND ND ND ND
incidence
Human exposure efficiency relative to U235 (IR) kBq U235 eq ND ND ND ND ND ND
Comparative toxic unit for ecosystems (ETP-fw) CTUe ND ND ND ND ND ND
Comparative toxic unit for humans (carcinogenic) (HTP-c) CTUh ND ND ND ND ND ND
Comparative toxic unit for humans (noncarcinogenic) (HTP-nc) CTUh ND ND ND ND ND ND
Soil quality index (SQP) SQP ND ND ND ND ND ND
The secondary
material (SM) used leads from paper production.
Disclaimer 2 –
for the indicators “abiotic depletion potential for non-fossil resources”,
“abiotic depletion potential for fossil resources”, “water (user) deprivation
potential, deprivation-weighted water consumption”, “potential comparative
toxic unit for ecosystems”, “potential comparative toxic unit for humans –
cancerogenic”, “Potential comparative toxic unit for humans - not
cancerogenic”, “potential soil quality index”.
The results of
this environmental impact indicator shall be used with care as the
uncertainties
on these results are high as there is limited experience with the
indicator.
6. LCA: Interpretation
The dominance analysis shows that the main causes for the respective environmental effects and indicators.
environmental impacts and indicators can be found in
information module A1. This shows the total global warming
potential for material provision at around 92%, based on all The reaction resin mixture itself accounts for 87% of the
information modules. With the total non-renewable primary total global warming potential in information module A1.
energy it is about 95%. Approx. 5% is accounted for by the PBT of the connector
and approx. 3% by the PP of the mixer.
Illustration:
Dominance analysis A1- A3
If you look at the material provision of the reaction resin
mixture and the packaging in detail, it becomes clear which Illustration:
raw materials make a decisive contribution to the Dominance analysis A1
9 Environmental-Product Declaration - Hilti AG - HIT-HY 170
Illustration:
Within the reaction resin mixture itself, about 40% of the Dominance analysis A1, reaction resin mixture
total global warming potential and about 39% of the total
non-renewable primary energy are created by the material
provision of the UMA 201. The HPMA has a share of
approx. 28% of the total greenhouse gas emissions and
approx. 30% of the total non-renewable primary energy.
7. Requisite evidence
As a general rule, all statements must be documented with
• DIBt (2010) in combination with the NIK values from
measured data (presented by the corresponding test
AgBB (2021) for applications in interior areas,
certificates). The methods of evidence and the test conditions
• emission class A+ outlined in the French VOC Directives
have to be described together with the results.
(2019) in accordance with the Eurofins attestation,
• CDPH/EHLB Standard Method V 1.2 (2017) in
If substances are not detected, the limit of detection must be
accordance with Eurofins test report, No. 392-2022-
included in the declaration.
00035301_C_EN, Eurofins test report, No. 392-2022-
00035301_E_EN and Eurofins test report, No. 392-
Interpreting statements such as “… free of …” or “… are
2022-00035302_H_EN respectively.
entirely harmless …” are not allowed.
AgBB overview of results (28 days [µg/m³])
If evidence required by the specific PCR part B is not provided, Name Value Unit
this has to be justified under the respective title for the required TVOC (C6 - C16) <1000 μg/m3
evidence.
Sum SVOC (C16 - C22) <100 μg/m3
If relevant for the scope of application of the declared product, R (dimensionless) <1 -
or if derivable from its material composition, it is recommended VOC without NIK <100 μg/m3
to provide additional adequate evidence.
Carcinogenic Substances <1 μg/m3
Hilti HIT-HY 170 complies with the requirements of
8. References
EN ISO 604 ISO 2811-1
EN ISO 604: 2003-12, Kunststoffe - Bestimmung von ISO 2811-1: 2016-08, Beschichtungsstoffe - Bestimmung der
Druckeigenschaften Dichte - Teil 1: Pyknometer-Verfahren
EN 13501-1 ISO 50001
EN 13501-1: 2019-05, Klassifizierung von Bauprodukten und ISO 50001: 2018-08, Energiemanagementsysteme -
Bauarten zu ihrem Brandverhalten - Teil 1: Klassifizierung mit Anforderungen mit Anleitung zur Anwendung
den Ergebnissen aus den Prüfungen zum Brandverhalten von ISO 527-1
Bauprodukten ISO 527-1: 2019-07, Kunststoffe - Bestimmung der
Zugeigenschaften - Teil 1: Allgemeine Grundsätze
EN 15804 ISO 9001
EN 15804+A2:2019+AC:2021, Sustainability of construction ISO 9001: 2015-11, Qualitätsmanagementsysteme -
works — Environmental Product Declarations — Core rules for Anforderungen
the product category of construction products
AgBB (2021)
Vorgehensweise bei der gesundheitlichen Bewertung der
ISO 14001 Emissionen von flüchtigen organischen Verbindungen (VVOC,
ISO 14001: 2015-09, Umweltmanagementsysteme - VOC und SVOC) aus Bauprodukten (2021)
Anforderungen mit Anleitung zur Anwendung
Candidate List of substances of very high concern for
Authorisation
ISO 14025 European Cheminals Agency (ECHA), in accordance with
DIN EN /ISO 14025:2011-10/, Environmental labels and Article 50(10) of the REACH regulation
declarations — Type III environmental declarations —
Principles and procedures
10 Environmental-Product Declaration - Hilti AG - HIT-HY 170
CDPH/EHLB/Standard Method V1.2 des peintures et vernis sur leurs émissions de polluants volatils
California CDPH Standard Method is a US standard for Arrêté du 19 avril 2011 relatif à l’étiquetage des produits de
evaluating and restricting VOC emissions to indoor air. construction ou de revêtement de mur ou de sol et des
Developed in California as "Section 01350" Specification, peintures et vernis sur leurs émissions de polluants volatils
several systems in the US refer to CDPH Standard Method
IBU 2021
Calculation rules: PCR - Part A
Institut Bauen und Umwelt e.V. (IBU), 2022. Product Category
Rules for Building-Related Products and Services. Part A: General
Calculation rules for the life cycle assessment and Instructions for the EPD programme of Institut Bauen und
requirements on the project report. Version 1.3 (08.2022) Umwelt e.V. Version
DIBt (2010) 2.0,
Grundsätze zur gesundheitlichen Bewertung von Bauprodukten
in Innenräumen (Oktober 2010)
ecoinvent 3.8 Berlin:
Backgroun data: ecoinvent 3.8 Institut Bauen und Umwelt e.V.,2021
Zürich: ecoinvent
http://www.ecoinvent.org
(28.09.2022)
www.ibu-epd.de
ETA 14/0457
European Technical Approval Hilti HIT-HY 170 Product category rules for construction products – Part B
ETA 15/0197
European Technical Approval Hilti HIT-HY 170
ETA 15/0297 Reaction resin products, 01.2019
European Technical Approval Hilti HIT-HY 170 Regulation (EU) No. 305/2011 (CPR)
Regulation (EU) No 305/2011 of the European Parliament and
of the Council of 9 March 2011 laying down harmonised
ETA 19/0161 conditions for the marketing of construction products and
European Technical Approval Hilti HIT-HY 170 repealing Council Directive 89/106/EEC Text with EEA
ETA 19/0465 relevance
European Technical Approval Hilti HIT-HY 170
Eurofins test report, No. 392-2022-00035301_C_EN
VOC test report for verification of compliance with Sphera
DIBt(2010)/AgBB(2021) GaBi 10
Software: Ganzheitliche Bilanzierung,
Eurofins test report, No. 392-2022-00035301_E_EN Leinfelden-Echterdingen;
VOC test report for verification of compliance with the French Sphera Solution GmbH,
directive from 2010 https://gabi.sphera.com/databases/gabi-data-search/
Eurofins test report, No. 392-2022-00035302_H_EN
VOC test report for verification of compliance with
CDPH/EHLB/Standard Method V1.2 from 2017
European Waste code
in accordance with the European Waste Catalogue (EWC)
(EWC 2014/955/EU) Commission Decision amending Decision
2000/532/EC on the list of waste pursuant to Directive
2008/98/EC of the European (28.09.2022)
Parliament and of the Council The literature referred to in the Environmental Product
Declaration must be listed in full.Standards already fully quoted
French VOC Directives in the EPD do not need to be listed here again.
Décret no 2011321 du 23 mars 2011 relatif à l’étiquetage des The current version of PCR Part A and PCR Part B of the PCR
produits de construction ou de revêtement de mur ou de sol et document on which they are based must be referenced.
11 Environmental-Product Declaration - Hilti AG - HIT-HY 170
Publisher
Institut Bauen und Umwelt e.V. +49 (0)30 3087748- 0
Hegelplatz 1 info@ibu-epd.com
10117 Berlin www.ibu-epd.com
Germany
Programme holder
Institut Bauen und Umwelt e.V. +49 (0)30 3087748- 0
Hegelplatz 1 info@ibu-epd.com
10117 Berlin www.ibu-epd.com
Germany
Author of the Life Cycle Assessment
FIT-Umwelttechnik GmbH 05362 72 69 474
Westerstr. 13 bertram@fit-umwelttechnik.de
38442 Wolfsburg www.fit-umwelttechnik.com
Germany
Owner of the Declaration
Hilti Aktiengesellschaft +423 234 2111
Feldkircher Strasse 100 HAGHSE@hilti.com
9494 Schaan www.hilti.com
Liechtenstein
12 Environmental-Product Declaration - Hilti AG - HIT-HY 170
