ENVIRONMENTAL PRODUCT DECLARATION
as per ISO 14025 and EN 15804+A2
Owner of the Declaration Knauf Ceiling Solutions GmbH & Co. KG
Publisher Institut Bauen und Umwelt e.V. (IBU)
Programme holder Institut Bauen und Umwelt e.V. (IBU)
Declaration number EPD-KNA-20220022-IBD2-EN
Issue date 30.03.2022
Valid to 29.03.2027
Mesh Ceiling Membranes (1.5 mm)
Knauf Ceiling Solutions GmbH & Co. KG
www.ibu-epd.com | https://epd-online.com
1. General Information
Knauf Ceiling Solutions GmbH & Co. KG Mesh Ceiling Membranes (1.5 mm)
Programme holder Owner of the declaration
IBU – Institut Bauen und Umwelt e.V. Knauf Ceiling Solutions GmbH & Co. KG
Hegelplatz 1 Elsenthal 15
10117 Berlin 94481 Grafenau
Germany Germany
Declaration number Declared product / declared unit
EPD­KNA­20220022­IBD2­EN 1 m² average mesh ceiling membrane for indoor application with a
thickness of 1.5 mm and a surface weight of 4.28 kg/m²
This declaration is based on the product category rules: Scope:
Metal ceilings, 01.08.2021 This document refers to average mesh ceiling membranes with a thickness
(PCR checked and approved by the SVR) of 1.5 mm and a surface weight of 4.28 kg/m².
The products are manufactured for Knauf Ceiling Solutions GmbH & Co.
Issue date KG at Italfim in Pedrengo (Italy).
30.03.2022
The owner of the declaration shall be liable for the underlying information
and evidence; the IBU shall not be liable with respect to manufacturer
information, life cycle assessment data and evidences.
Valid to
29.03.2027 The EPD was created according to the specifications of EN 15804+A2. In
the following, the standard will be simplified as EN 15804.
Verification
The standard EN 15804 serves as the core PCR
Independent verification of the declaration and data according to ISO
14025:2011
internally X externally
Dipl.­Ing. Hans Peters
(Chairman of Institut Bauen und Umwelt e.V.)
Florian Pronold Matthias Schulz,
(Managing Director Institut Bauen und Umwelt e.V.) (Independent verifier)
1 Environmental Product Declaration ­ Knauf Ceiling Solutions GmbH & Co. KG ­ Mesh Ceiling Membranes (1.5 mm)
2. Product
treated product as defined by the (EU) Ordinance on Biocide
2.1 Product description/Product definition Products No. 528/2012': No.
Knauf Ceiling Solutions mesh ceiling systems are made from
punched and formed galvanised steel, as comprehensive 2.6 Manufacture
construction kits or individual components and industrially The system components for mesh ceilings are manufactured in
manufactured. The construction kit comprises the visible a continuous manufacturing process. The sheet steel comes in
membrane and the substructure. The membranes (tiles, panels, coils, gets expanded, afterwards cut to size, punched, formed
bulkheads) are offered with various edge details and delivered and powder­coated after the cleaning process. Punching waste
with a range of mesh patterns, fulfilling the functional is gathered, collected by local disposal companies, and
requirements. The substructure is either exposed or concealed. redirected to the recycling centres. All production steps are
carried out in accordance with the requirements and test
For the placing on the market of the product in the European guidelines outlined in EN 13964.
Union/European Free Trade Association (EU/EFTA) (with the
exception of Switzerland) Regulation (EU) No. 305/2011 (CPR) The manufacturing plant is certified according to ISO 9001.
applies. The product needs a declaration of performance taking
into consideration EN 13964:2014, suspended ceiling 2.7 Environment and health during manufacturing
requirements and test methods and the CE­marking and Manufacturing conditions do not demand any particular health
UKCA­marking (in the UK). protection measures with the exception of those designated by
For the application and use the respective national provisions the authorities for special working areas, e.g., high­visibility
apply. vests, ear protection, safety shoes.
The threshold limit values are not exceeded at any point in the
2.2 Application production process. Waste emissions generated during
The described meshsolutions are typically used internally as production are cleaned in accordance with statutory
design elements, to cover the ceiling void, as well as acoustic requirements. Emissions are below those outlined in the
solutions for sound absorption and sound attenuation, for fire Technical Guidelines governing Air. Water/ground: No
resistance and against fire spreading, for cleanrooms and high contamination of water or soil occurs. Noise­intensive plant
hygiene requirements. components such as mesh expansion lines are isolated
accordingly by structural measures.
2.3 Technical Data
Mesh membranes are regulated by EN 13964 and have 2.8 Product processing/Installation
corresponding labelling and declaration of performance. There are no recognised systemic hazards associated with the
The following data provide an overview of results: installation of ceiling membranes. Mesh ceiling membranes are
suspended by a substructure.
Constructional data
Installation must be carried out by trained personnel. Workers
Name Value Unit
should wear appropriate personal protective equipment.
Grammage 4.28 kg/m2 Equipment such as gloves and goggles are recommended to
Release of formaldehyde (EN 13964) E1 ­ prevent skin irritation.
Durability class (EN 13964) C ­
2.9 Packaging
Further characteristics according to the PCR are not relevant The membranes are packaged in cardboard boxes, panels and
for this product. bulkheads in wooden crates. These packages lie on chemically
untreated wooden pallets and are easily separable. The pallets
The performance data of the product, with respect to its are wrapped with polyethylene stretch film. Film, paper and
essential characteristics, is in accordance with the declaration wood can be recycled in the usual ways.
of performance according to EN 13964:2014, suspended
ceiling requirements and test methods. 2.10 Condition of use
Long service life is based on regular maintenance, care and
2.4 Delivery status repair of the product. When handled properly, the mechanical
The mesh ceiling systems, construction kits and components and structural physical properties of the mesh membrane
are produced in individual module sizes and can be supplied remain intact throughout its entire service life. Generally, the
with or without substructures. material composition of the product does not alter during the
Packaging is usually on pallets and/or in cardboard. period of use.
2.5 Base materials/Ancillary materials 2.11 Environment and health during use
Name Value Unit There are no known interactions between the product, the
Galvanised steel > 95.5 % environment and health. Volatile organic compounds are below
the valuation limit.
Surface coating < 4.5 %
1) 'This product contains substances listed in the candidate list 2.12 Reference service life
(08.07.2021) exceeding 0.1 percentage by mass': No. The service life of the mesh membranes is for more than 50
years, depending on the area of use, exposure and state of
2) 'This product contains other carcinogenic, mutagenic, maintenance. Within the framework of the conditions of use, no
reprotoxic (CMR) substances in categories 1A or 1B which are ageing effects are to be expected apart from visual
not on the candidate list, exceeding 0.1 percentage by mass': discolouration caused by air circulation.
No.
2.13 Extraordinary effects
3) 'Biocide products were added to this construction product or Fire
it has been treated with biocide products (this then concerns a The declared products are classified in the fire reaction class
2 Environmental Product Declaration ­ Knauf Ceiling Solutions GmbH & Co. KG ­ Mesh Ceiling Membranes (1.5 mm)
A2­s1, d0 according to EN 13501-1. This means that they are In the case of mechanical destruction, all substances remain
"non­combustible" according to the German building authority bound. It can be assumed that in the case of coated ceilings,
designation (and also many other European countries) with possible paint splinters arise in such small volumes that no
negligible smoke development and no burning droplets in the negative effects are incurred by the environment.
event of a fire.
2.14 Re-use phase
Fire reaction
The mesh ceiling systems can be removed and re­used without
Name Value damaging the product. Mesh membrane components and
Building material class A2 substructure components made of steel can be redirected to
Burning droplets s1 material recycling.
Smoke gas development d0
2.15 Disposal
In accordance with the Waste Index Act (AVV) and the
Water European Waste Catalogue (EWC), the waste key for steel as a
No environmental influences are known in the case of component of mesh ceiling systems made of steel is: 17­04­05
unforeseen water ingress. The resistance of the ceiling system – Iron and steel.
following the impact of water is dependent on the corrosion
protection class in which the ceiling system is classified. 2.16 Further information
Further information at www.knaufceilingsolutions.com
Mechanical destruction
3. LCA: Calculation rules
as the site's own photovoltaic plant.
3.1 Declared Unit
This EPD refers to a declared unit of 1 m² of average mesh The packaging of the products is considered in this stage.
ceiling membrane with a thickness of 1.5 mm (Standard white
RAL 9010) and a surface weight of 4.28 kg/m². Module C1 | Deconstruction and demolition
Declared unit Disassembly of the product is done either manually or using
smaller tools. Referring energy demand is considered to be
Name Value Unit
negligible.
Declared unit 1 m2
Grammage 4.28 kg/m2 Module C2 | Transport to disposal
The transport to the disposal of the material is estimated
The substructure is not part of this EPD.
declaring a 50 km radius to the disposal. In reality, this scenario
may vary depending on the actual location of deconstruction
The mesh ceiling membranes are produced under different
and referring waste treatment.
brand names, for Knauf Ceiling Solutions at Italfim in Pedrengo
(IT). The declared product represents an average based on the
Module C3 | Waste processing
production volume.
Regarding the steel fraction, the material flow reaching module
D for recycling is declared as material for recycling in Module
Knauf Ceiling Solutions mesh ceiling membranes can be
C3. Environmental impacts resulting from the grinding and
specifically configurated based on the customer's need
sorting of steel scrap are not included. In addition, a loss rate of
resulting in more than 20 standard products. The declared unit,
5 % of the processed material is assumed. 95 % of the material
therefore, refers to a representative product sold in large
can potentially be recycled.
quantities. Products are available in various pattern designs
such as RB35 and RB55 and further mesh patterns. The
Module C4 | Disposal
declared average results out of the weighting of the products
Module C4 refers to the emissions from the disposal of the
RB35 and RB55 with a steel gauge of 1.5 mm.
losses from waste processing of lost steel. The chosen
scenario, therefore, includes the environmental burdens of
As the mass of steel represents the decisive factor in the
landfilling of 5 % of the mesh material.
product's environmental profile, a linear correlation of product
mass and environmental impact is to be expected. Thus, the
Module D | Benefits and loads beyond the system
recalculation for specific products based on the product mass is
boundary
possible.
Module D declares the recycling of the recovered steel (95 % of
3.2 System boundary the product). It includes the potential for substituting primary
steel.
The life cycle assessment of average mesh ceiling membranes
includes a cradle­to­gate analysis of the products'
3.3 Estimates and assumptions
environmental impacts with modules C1–C4 and module D
Assumptions and approximations are applied in case of a lack
(A1–A3, + C + D). Subsequent life cycle phases are part of the
of representative data. All assumptions and approximations are
analysis:
documented precisely and represent a best­guess
representation of reality. In case of uncertainty, a conservative
Module A1-A3 | Production stage
approach is chosen.
The production stage includes the upstream burdens of raw
material supply, their transports and the manufacturing plant of 3.4 Cut-off criteria
Italfim located in Pedrengo (IT). The production of mesh ceiling
The LCA model covers all available input and output flows,
membranes includes punching and trimming, powder coating
which can be represented based on robust data. Data gaps are
and packaging. Main raw material inputs, therefore, refer to
filled with conservative assumptions from average data (when
steel and paint for powder coating. The production site in
available) or with generic data and are documented
Pedrengo is supplied with electricity from the Italian grid as well
3 Environmental Product Declaration ­ Knauf Ceiling Solutions GmbH & Co. KG ­ Mesh Ceiling Membranes (1.5 mm)
accordingly. Only data with a contribution lower than 1 % were Land or region, in which the declared product system is
cut off. Thus, no data were neglected, of which a substantial manufactured, used or handled at the end of the product´s
impact is to be expected. All relevant data were collected lifespan: Italy
comprehensively. Cut­off material and energy flows were
chosen carefully based on their expected quantitative
contribution as well as potential environmental impacts. Thus, it 3.9 Allocation
can be assumed that the sum of all neglected input flows does For foreground data, the calculation of specific input quantities
not account for more than 5 % of the total material, water and is based on the annual production quantity (square meter), e.g.
energy flows. for energy input, packaging, etc.. The steel input on product
level was calculated based on the mass of steel in the output.
3.5 Background data
This study uses generic background data for the evaluation of Background data for the supply chain of the steel are published
upstream environmental impacts from GaBi databases (GaBi by worldsteel (GaBi-databases). Representing an average of
10; 2021.2). the global steel industry, worldsteel background datasets
ensure a good geographical and technological representation
3.6 Data quality
of steel production. All worldsteel datasets are modelled
Data collection is based on product­specific questionnaires. It according to the worldsteel LCA methodology, applying the
follows an iterative process clarifying questions via e­mail, system expansion approach for the allocation of co­products
telephone calls or in personal/web meetings. Intensive from steel production. As a result, these datasets are not fully
discussions between Knauf Ceiling Solutions and Daxner & compliant with the requirements of the EN 15804, which
Merl results in an accurate mapping of product­related material emphasises the so­called partitioning approach applying a
and energy flows. This leads to a high quality of foreground subdivision of environmental impacts according to their physical
data collected. Data collection relies on a consistent process relationships. Due to a lack of global data calculated based on
according to ISO 14044. the partitioning approach, the worldsteel datasets refer to the
closest representation of steel production in this context.
The technological, geographical and time­related Additionally, the deviation of the results of the two allocation
representativeness of the database was kept in mind when approaches is to be expected under 5 % according to Sphera.
selecting background data. Whenever specific data were Scrap input is regarded as burden­free.
missing, either generic datasets or representative average data
were used instead. The implemented GaBi background 3.10 Comparability
datasets refer to the latest versions available (not more than Basically, a comparison or an evaluation of EPD data is only
ten years old) and are carefully chosen. possible if all the data sets to be compared were created
according to EN 15804 and the building context, respectively
3.7 Period under review
the product­specific characteristics of performance, are taken
Foreground data were collected for the production year 2020. into account.
The data are based on the volumes produced on an annual The GaBi background database was used to calculate the LCA
basis. (GaBi 10; 2021.2).
3.8 Geographic Representativeness
4. LCA: Scenarios and additional technical information
End of life (C1-C4)
Characteristic product properties of biogenic carbon
Name Value Unit
Information on describing the biogenic Carbon Content at
Collected separately (steel) 4.28 kg
factory gate
Recycling 95 % 4.07 kg
Name ValueUnit
Landfilling 5 % 0.21 kg
Biogenic carbon content in accompanying kg
0.1
packaging C
Reuse, recovery and/or recycling potentials (D), relevant
The declared product does not contain biogenic carbon. scenario information
Name Value Unit
Net flow of steel scrap 3.85 kg/m²
4 Environmental Product Declaration ­ Knauf Ceiling Solutions GmbH & Co. KG ­ Mesh Ceiling Membranes (1.5 mm)
5. LCA: Results
The following table contains the LCA results for a declared unit of 1 m² average mesh ceiling membrane with a thickness of 1.5 mm
and a surface weight of 4.28 kg/m².
Disclaimer:
EP­freshwater: This indicator has been calculated as 'kg P eq' as required in the characterization model (EUTREND model, Struijs et
al., 2009b, as implemented in ReCiPe; http://eplca.jrc.ec.europa.eu/LCDN/developerEF.xhtml).
DESCRIPTION OF THE SYSTEM BOUNDARY (X = INCLUDED IN LCA; ND = MODULE OR INDICATOR NOT DECLARED; MNR =
MODULE NOT RELEVANT)
Benefits and
Construction loads beyond
Product stage Use stage End of life stage
process stage the system
boundaries
la ire ta m w a Ry lp p u s tro p s n a rT g n iru tc a fu n a M e h t m o rf tro p s n a rTe tis e h t o t e ta g y lb m e s s A e s U e c n a n e tn ia M ria p e R tn e m e c a lp e R tn e m h s ib ru fe R y g re n e la n o ita re p Oe s u re ta w la n o ita re p Oe s u n o itc u rts n o c ­e Dn o itilo m e d tro p s n a rT g n is s e c o rp e ts a W la s o p s iD ­e s u e R­y re v o c e R­g n ilc y c e Rla itn e to p
A1 A2 A3 A4 A5 B1 B2 B3 B4 B5 B6 B7 C1 C2 C3 C4 D
X X X MND MND MND MND MNR MNR MNR MND MND X X X X X
RESULTS OF THE LCA - ENVIRONMENTAL IMPACT according to EN 15804+A2: 1 m² mesh ceiling membrane (1.5 mm; 4.28
kg/m²)
Parameter Unit A1-A3 C1 C2 C3 C4 D
Global Warming Potential total (GWP­total) kg CO 2 eq 1.39E+01 0 1.29E­02 0 1.04E­02 ­6.54E+00
Global Warming Potential fossil fuels (GWP­fossil) kg CO 2 eq 1.47E+01 0 1.29E­02 0 1.05E­02 ­6.54E+00
Global Warming Potential biogenic (GWP­biogenic) kg CO 2 eq ­7.94E­01 0 ­1.52E­05 0 ­1.07E­04 ­3.72E­03
Global Warming Potential luluc (GWP­luluc) kg CO 2 eq 5.6E­03 0 1.05E­04 0 1.05E­05 ­1.43E­04
Depletion potential of the stratospheric ozone layer (ODP) kg CFC11 eq 3.64E­12 0 2.53E­18 0 2.47E­17 ­1.56E­14
Acidification potential of land and water (AP) mol H+ eq 3.81E­02 0 4.24E­05 0 3.33E­05 ­1.16E­02
Eutrophication potential aquatic freshwater (EP­freshwater) kg P eq 1.41E­05 0 3.8E­08 0 7.95E­09 ­1.42E­06
Eutrophication potential aquatic marine (EP­marine) kg N eq 9.32E­03 0 1.95E­05 0 8.26E­06 ­2.24E­03
Eutrophication potential terrestrial (EP­terrestrial) mol N eq 9.94E­02 0 2.18E­04 0 9.07E­05 ­2.27E­02
Formation potential of tropospheric ozone photochemical oxidants kg NMVOC
3.03E­02 0 3.83E­05 0 2.6E­05 ­1E­02
(POCP) eq
Abiotic depletion potential for non fossil resources (ADPE) kg Sb eq 5.93E­05 0 1.13E­09 0 7.21E­10 ­1.62E­05
Abiotic depletion potential for fossil resources (ADPF) MJ 1.75E+02 0 1.7E­01 0 1.52E­01 ­6.4E+01
m3 world eq
Water use (WDP) 2.08E+01 0 1.19E­04 0 ­1.24E­04 ­1.78E+01
deprived
RESULTS OF THE LCA - INDICATORS TO DESCRIBE RESOURCE USE according to EN 15804+A2: 1 m² mesh ceiling
membrane (1.5 mm; 4.28 kg/m²)
Parameter Unit A1-A3 C1 C2 C3 C4 D
Renewable primary energy as energy carrier (PERE) MJ 1.33E+01 0 9.81E­03 0 1.1E­02 4.02E+00
Renewable primary energy resources as material utilization
MJ 8.02E+00 0 0 0 0 0
(PERM)
Total use of renewable primary energy resources (PERT) MJ 2.13E+01 0 9.81E­03 0 1.1E­02 4.02E+00
Non renewable primary energy as energy carrier (PENRE) MJ 1.72E+02 0 1.71E­01 0 1.52E­01 ­6.4E+01
Non renewable primary energy as material utilization (PENRM) MJ 3.17E+00 0 0 ­3.01E+00 0 0
Total use of non renewable primary energy resources (PENRT) MJ 1.75E+02 0 1.71E­01 ­3.01E+00 1.52E­01 ­6.4E+01
Use of secondary material (SM) kg 4.76E­01 0 0 0 0 3.85E+00
Use of renewable secondary fuels (RSF) MJ 0 0 0 0 0 0
Use of non renewable secondary fuels (NRSF) MJ 0 0 0 0 0 0
Use of net fresh water (FW) m3 4.97E­01 0 1.12E­05 0 1.57E­06 ­4.16E­01
RESULTS OF THE LCA – WASTE CATEGORIES AND OUTPUT FLOWS according to EN 15804+A2:
1 m² mesh ceiling membrane (1.5 mm; 4.28 kg/m²)
Parameter Unit A1-A3 C1 C2 C3 C4 D
Hazardous waste disposed (HWD) kg 1.62E­07 0 9.01E­12 0 2.7E­11 1.4E­08
Non hazardous waste disposed (NHWD) kg 4.26E­01 0 2.68E­05 0 2.14E­01 8.16E­01
Radioactive waste disposed (RWD) kg 1.83E­03 0 3.1E­07 0 1.73E­06 6.94E­06
Components for re­use (CRU) kg 0 0 0 0 0 0
Materials for recycling (MFR) kg 0 0 0 4.07E+00 0 0
Materials for energy recovery (MER) kg 0 0 0 0 0 0
Exported electrical energy (EEE) MJ 0 0 0 0 0 0
Exported thermal energy (EET) MJ 0 0 0 0 0 0
5 Environmental Product Declaration ­ Knauf Ceiling Solutions GmbH & Co. KG ­ Mesh Ceiling Membranes (1.5 mm)
RESULTS OF THE LCA – additional impact categories according to EN 15804+A2-optional:
1 m² mesh ceiling membrane (1.5 mm; 4.28 kg/m²)
Parameter Unit A1-A3 C1 C2 C3 C4 D
Disease
Incidence of disease due to PM emissions (PM) 5.32E­07 0 2.41E­10 0 3.61E­10 ­2.21E­07
incidence
Human exposure efficiency relative to U235 (IR) kBq U235 eq 4.28E­01 0 4.54E­05 0 2.49E­04 1.21E­01
Comparative toxic unit for ecosystems (ETP­fw) CTUe 3.1E+01 0 1.26E­01 0 4.48E­02 ­4.13E+00
Comparative toxic unit for humans (carcinogenic) (HTP­c) CTUh 6.32E­09 0 2.56E­12 0 5.2E­12 ­3.55E­09
Comparative toxic unit for humans (noncarcinogenic) (HTP­nc) CTUh 1.91E­07 0 1.5E­10 0 5.22E­10 ­7.89E­08
Soil quality index (SQP) SQP 1.55E+02 0 5.86E­02 0 1.12E­02 9.59E­01
Disclaimer 1 – for the indicator “Potential Human exposure efficiency relative to U235”. This impact category deals mainly with the
eventual impact of low­dose ionizing radiation on human health of the nuclear fuel cycle. It does not consider effects due to possible
nuclear accidents, occupational exposure or radioactive waste disposal in underground facilities. Potential ionizing radiation from the
soil, radon and from some construction materials is also not measured by this indicator.
Disclaimer 2 – for the indicators “abiotic depletion potential for non­fossil resources”, “abiotic depletion potential for fossil resources”,
“water (user) deprivation potential, deprivation­weighted water consumption”, “potential comparative toxic unit for ecosystems”,
“potential comparative toxic unit for humans – cancerogenic”, “Potential comparative toxic unit for humans ­ not cancerogenic”,
“potential soil quality index”. The results of this environmental impact indicator shall be used with care as the uncertainties on these
results are high as there is limited experience with the indicator.
6. LCA: Interpretation
The following interpretation contains a summary of the LCA weight of 4.28 kg/m² produced for Knauf Ceilings Solutions at
results referenced to a declared unit of 1 m² of average mesh Italfim in Pedrengo (IT).
ceiling membrane with a thickness of 1.5 mm and a surface
The comparison of the products' life cycle phases shows a phase of the mesh membranes, the upstream supply chain of
clear dominance of the production phase (modules A1­A3). the steel coils represents the major hot spot in all of the impact
categories considered, except for potential ozone depletion.
Module C4 declares impacts from landfilling of steel losses
(assumption: 5 % of steel in the product) making up a minor Furthermore, the coating has an observable influence on total
fraction of the total environmental impact of the products. global warming potential (GWP­total) as well as abiotic
depletion potential for fossil resources (ADPF).
As a result of material recyclability, the steel fraction removed at
the end of life can substitute primary steel. Module D shows the Knauf Ceiling Solutions mesh ceiling membranes can be
recycling potential of 95 % of the steel in the product at the end specifically configurated based on the customer's need
of its life. This results in credits from the substitution of primary resulting in more than 20 standard products. The conversion of
steel. the LCA results to other material thicknesses than the declared
reference thickness is principally proportional to the surface
When it comes to the environmental impacts in the production weight. As a result, the variability of the environmental impacts
6 Environmental Product Declaration ­ Knauf Ceiling Solutions GmbH & Co. KG ­ Mesh Ceiling Membranes (1.5 mm)
of single products shows a direct correlation to the steel content of the product.
7. Requisite evidence
The relevant paragraph of the suspended ceiling product containing compound is used during the manufacturing
standard (EN 13964) requires formaldehyde emissions process. Mesh ceilings covered by this EPD do not contain any
declaration only for products for which a formaldehyde­ formaldehyde­containing compounds.
8. References
Standards authorisation (ECHA Candidate List), 25.06.2020, published
under Article 59(10) of REACH. Helsinki:
EN 13501-1 European Chemicals Agency.
EN 13501­1:2019, Classification of construction products and
building elements according to their reaction to fire, Part 1: European Waste Catalogue
Classification with the results of tests on the reaction to fire of Guidance on classification of waste according to EWC­Stat
construction products. categories. Supplement to the Manual for the Implementation of
the Regulation (EC) No 2150/2002 on Waste Statistics.
EN 13964 Commission of the European Communities, EUROSTAT.
EN 13964:2014, Suspended ceilings ­ Requirements and test
methods. GaBi
GaBi 10, Software­System and Database for Life Cycle
EN 15804 Engineering. DB 2021.2. Stuttgart, Echterdingen: Sphera,
EN 15804:2012+A2:2019, Sustainability of construction works ­ 1992­2021. Available at:
Environmental product declarations ­ Core rules for the product http://documentation.gabi­software.com
category of construction products.
IBU 2021
ISO 9001 Institut Bauen und Umwelt e.V.: Allgemeine Anleitung für das
EN ISO 9001:2015­11, Quality management systems ­ EPD­­Programm des Institut Bauen und Umwelt e.V. (IBU).
Requirements. Version 2.0, Berlin: Institut Bauen und Umwelt e.V., 2021.
www.ibu­­epd.com
ISO 14025
DIN EN ISO 14025:2011­10, Environmental labels and Ordinance on Biocide Products
declarations ­ Type III environmental declarations ­ Principles Regulation (EU) No 528/2012 of the European Parliament and
and procedures. of the Council of 22 May 2012 concerning the making available
on the market and use of biocidal products.
ISO 14044
EN ISO 14044:2006­10, Environmental management – Life PCR part A
cycle assessment – Requirements and guidelines. Product category rules for building­­related products and
services. Part A: Calculation Rules for the Life Cycle
Further References Assessment and Requirements on the Project Report according
to EN 15804+A2:2019. Version 1.1.
AVV Berlin: Institut Bauen und Umwelt e.V., 2021.
AVV, German List of Wastes Ordinance. Regulation on the
European Waste List. PCR: Metal ceilings
Product category rules for building­related products and
Candidate list services. Part B: EPD requirements for metal ceilings. Version
List of substances of very high concern (SVHC) for 1.7. Berlin: Institut Bauen und Umwelt e.V., 08.01.2019.
7 Environmental Product Declaration ­ Knauf Ceiling Solutions GmbH & Co. KG ­ Mesh Ceiling Membranes (1.5 mm)
Publisher
Institut Bauen und Umwelt e.V. +49 (0)30 3087748­ 0
Hegelplatz 1 info@ibu­epd.com
10117 Berlin www.ibu­epd.com
Germany
Programme holder
Institut Bauen und Umwelt e.V. +49 (0)30 3087748­ 0
Hegelplatz 1 info@ibu­epd.com
10117 Berlin www.ibu­epd.com
Germany
Author of the Life Cycle Assessment
Daxner & Merl GmbH +43 676 849477826
Lindengasse 39/8 office@daxner­merl.com
1070 Wien www.daxner­merl.com
Austria
Owner of the Declaration
Knauf Ceiling Solutions GmbH & Co. KG 0049 8552 422 0
Elsenthal 15 ceiling.solutions@knauf.com
94481 Grafenau www.knaufceilingsolutions.com
Germany
8 Environmental Product Declaration ­ Knauf Ceiling Solutions GmbH & Co. KG ­ Mesh Ceiling Membranes (1.5 mm)
