ENVIRONMENTAL PRODUCT DECLARATION
as per ISO 14025 and EN 15804+A2
Owner of the Declaration Armacell GmbH
Programme holder Institut Bauen und Umwelt e.V. (IBU)
Publisher Institut Bauen und Umwelt e.V. (IBU)
Declaration number EPD-ARM-20200220-IBA1-EN
Issue date 12.03.2021
Valid to 11.03.2026
NH/ArmaFlex insulation for building equipment and industrial
installations
Armacell GmbH
www.ibu-epd.com | https://epd-online.com
Umwelt Produktdeklaration Name des Herstellers – Name des Produkts
1. General Information
Armacell GmbH NH/ArmaFlex
Programme holder Owner of the declaration
IBU – Institut Bauen und Umwelt e.V. Armacell GmbH
Panoramastr. 1 Robert-Bosch-Str. 10
10178 Berlin 48153 Münster - Germany
Germany
Declaration number Declared product / declared unit
EPD-ARM-20200220-IBA1-EN 1m³ insulation material NH/ArmaFlex
This declaration is based on the product Scope:
category rules: Product line NH/ArmaFlex
Insulating materials made of foam plastics, 06.2017 Insulation material for industrial and building
(PCR checked and approved by the SVR) installations vulcanized in tubes and sheets.
This declaration is an Environmental Product
Issue date Declaration according to ISO 14025 describing the
12.03.2021 specific environmental performance of the product
produced in Germany.
Valid to
11.03.2026 As the installation of the product is not restricted to
countries where the products have been produced the
validity of this EPD is considered at least EU wide.
The owner of the declaration shall be liable for the
underlying information and evidence; the IBU shall not
be liable with respect to manufacturer information, life
cycle assessment data and evidences.
The EPD was created according to the specifications
of EN 15804+A2. In the following, the standard will be
simplified as EN 15804.
Verification
The standard EN 15804 serves as the core PCR
Independent verification of the declaration and data
according to ISO 14025:2010
Dipl. Ing. Hans Peters internally x externally
(chairman of Institut Bauen und Umwelt e.V.)
Dr. Alexander Röder Mr Carl-Otto Neven
(Managing Director Institut Bauen und Umwelt e.V.)) (Independent verifier)
2. Product
2.1 Information about the enterprise automotive, wind energy, sports and
Armacell International GmbH is a producer of flexible construction.
insulation foams for the equipment insulation market
and a provider of engineered foams which operates
The product focus is insulation materials enhancing the
two main businesses:
energy efficiency of technical equipment, high-
 Advanced Insulation develops flexible foams
performance foams for technical and lightweight
for the insulation of technical equipment
applications, 100% recycled PET products and next-
utilised for the transport of energy - such as
generation aerogel technology.
heating, ventilation & air conditioning (HVAC)
and heating & plumbing (H&P) in residential 2.2 Product description/Product definition
and commercial construction, process lines in NH/ArmaFlex is the professional, highly-flexible,
closed-cell elastomeric foam insulation (FEF) for
the heavy- and oil & gas industry, equipment
continuous energy saving and condensation control
in transportation, as well as, acoustics.
purposes. The combination of very low thermal
 Engineered Foams develops high-
conductivity and high resistance to water vapour
performance foams for the use in a broad transmission prevents long-term energy losses and
range of end markets including transportation, water vapour ingress and reduces the risk of corrosion
under insulation.
2 Environmental Product Declaration Armacell GmbH – NH/ArmaFlex insulation for industrial and building installation
common pipe diameters up to an outer diameter of 114
For the placing on the market of the product in mm (tubes).
the European Union/European Free Trade Association
(EU/EFTA) (with the exception of Switzerland) 2.6 Base materials/Ancillary materials
Regulation (EU) No. 305/2011 (CPR) applies. The
product needs a declaration of performance taking into ArmaFlex is a highly flexible insulation material based
consideration EN 14304:2013-04 and the CE-marking. on synthetic rubber, which consists of around 20 basic
For the application and use the respective national components. The following table displays the
provisions apply. composition split into functional substance groups.
2.3 Application Name Value Unit
NH/ArmaFlex is used to insulate pipes, air ducts and Rubber and polymers 18 %
vessels including fittings and flanges of industrial Fillers and pigments 4 %
installations and building equipment. Blowing agent 11 %
 Condensation control, energy saving and Vulcanisation system, additives,
26 %
noise control in refrigeration and air plasticisers
conditioning equipment and process plants. Flame retardant 41 %
 Energy saving according to local energy-
Synthetic rubber determines the flexibility;
saving laws, prevention of heat loss and noise
Fillers determine the fire properties and firmness;
reduction of heating and plumbing systems.
Blowing agent causes the expansion process during
 Condensation control and noise reduction in manufacturing;
service-water and waste-water systems. Accelerator and sulphur enable the vulcanisation;
 Condensation control, energy saving and Plasticizers determine the flexibility;
Flame retardants ensure fire resistance.
noise control in refrigeration and air-
conditioning equipment in the ship-building
According to the European Chemicals Regulation
sector.
REACH manufacturer, importers and downstream
users must register their chemicals and are
responsible for their safe use on their own. For its
2.4 Technical Data production Armacell uses exclusively verifiably
registered and approved substances / mixtures.
According to available data and the information
Constructional data provided by preliminary suppliers, the product does not
Name Value Unit contain substances (SVHC) that are considered
Gross density 62.5 kg/m3 substances meeting the criteria for inclusion in annex
Water vapour diffusion resistance XIV (List of Substances Subject to Authorisation) as
≥ 2000 -
factor acc. to EN 12086, EN13469 laid down in Article 57 and article 59 of REACH (EC)
0,040 1907/2006.). Products manufactured and marketed by
Thermal conductivity (0°C) W/(mK) Armacell do not have to be registered. The products
may contain traces of azodicarbonamide (ACDA).
Maximum service temperature
+110 °C Possible minimal residual amounts are included in the
acc. to EN 14706, EN 14707
polymer matrix. A health impairment can be excluded.
Minimum service temperature -50 °C
For the production of insulation material based on
Tubes: DL-
Reaction to fire acc. to EN 13501- synthetic rubber, there is presently no alternative to
s2, d0/ -
1 ADCA available.
Sheets: E
Structure-borne sound
not
transmission acc. to EN ISO
relevant 2.7 Manufacture
3822-1
ArmaFlex products are manufactured in a
Weighted sound absorption
not pressureless, continuous and discontinuous production
coefficient αw acc. to EN ISO
relevant process.
11654
In the first step, a homogenous compound is produced
with rubber, additives, ancillary materials, blowing and
Insulation materials on the basis of synthetic rubber do
vulcanization agents. This is done on the rolling mill or
not absorb moisture from the air. For this reason the
in the internal mixer followed by the rolling mill.
normal building moisture does not lead to an increase
Rubber extruders are used to process the compounds
in thermal conductivity.
to produce raw profiles with defined dimensions. Here
exact compliance with the dimensions for the raw
Performance data of the product in accordance with
profile is crucial for the dimensional accuracy of the
the declaration of performance with respect to its
foamed product.
essential characteristics according to EN 14304:2013-
In the case of the discontinuous, pressureless
04
production process, the raw profiles are cut to length
and then foamed in a hot-air oven. In the case of the
2.5 Delivery status
continuous, pressureless process, the extruded profile
Halogen free FEF made of cross-linked elastomer is
is fed directly onto a vulcanization line whose energy
supplied as sheets, tubes and shaped pieces.
source may be hot air, for example.
Products with self-adhesive backings/closures are
In foam production, vulcanization and blowing
available; these variations are not included in the
processes run alongside each other. Both reactions
calculations. Insulation thicknesses are available for all
are regulated by temperature control. Recipe and
3 Environmental Product Declaration Armacell GmbH – NH/ArmaFlex insulation for industrial and building installation
temperature control determine the properties of the It is practically only restricted by the service life of the
foam. equipment or whole building, which can extent that
Quality assurance: time period. The insulation performance is almost
EC Certificate of conformity no. 0543 of the completely maintained over the entire service life. The
Gütegemeinschaft Hartschaum e.V. Celle. insulation performance is only compromised by
Quality management system in accordance with EN extraordinary impacts and damage during construction,
ISO 9001.
2.8 Environment and health during 2.14 Extraordinary effects
manufacturing
During all manufacturing steps and at all production Fire
sites of Armacell, the production follows the national According to EN 13501, ArmaFlex is classified as a
guidelines and regulations. A regenerative thermal combustible insulation material. Due to its material
oxidizer is installed to treat exhaust air. structure ArmaFlex does not contribute to an
Certification of the environmental management system uncontrollable spread of fire under installation
is in accordance with ISO 14001. conditions typical on a building site. ArmaFlex does not
drip under practical fire conditions, this means that fire
spread is ruled out. The product is self-extinguishing
2.9 Product processing/Installation and therefore only makes a minor contribution to the
The product is installed by using knives. No special actual fire event. There is no possibility of the material
tools, nor specific protection is necessary. self-igniting. ArmaFlex does not propagate the fire
When applying adhesives the information given in the either horizontally or vertically.
relevant safety data sheets is to be heeded.
The recommendations for installing the product Fire protection
depend on the product and system and are described Name Value
in the respective documents (e.g. Armaflex application Tubes: DL
manual) or the data sheets. More details under Euro class / Sheets:
www.armacell.com. E
Tubes: d0
Burning droplets
/ Sheets: -
2.10 Packaging Tubes: s2
Smoke development
As a rule, ArmaFlex products are packaged in / Sheets: -
cardboard boxes and transported on reusable pallets.
Over-sized rolls of sheet material are packaged Water
in polyethylene (PE) foil. The cardboard boxes can be Armacell insulation materials have a high resistance to
recycled through Interseroh’s dual system. water vapour transmission which keeps possible water
vapour transmission processes to a minimum
permanently. Therefore, a significant reduction in the
2.11 Condition of use insulation effect can be ruled out permanently.
When the products are used for the purpose for which If the insulation material is exposed to water over a
they are intended, there are no changes in the material long period of time (e.g. flooding) it should be replaced.
composition during use, except in the event of
extraordinary impacts (see 2.14). Mechanical destruction
ArmaFlex insulation materials are flexible foams and
2.12 Environment and health during use thus display limited mechanical stability. Therefore, if
Ingredients: There are no particular aspects of the the material will be subject to greater mechanical
material composition during use. impact it should be protected appropriately, e.g. by a
Eurofins Product Testing A/S has tested a wide range metal jacket or Arma-Chek covering.
and varieties of typical FEF (Flexible Elastomeric ArmaFlex products (with the exception of
Foam) products marketed in the EU from CEFEP HT/ArmaFlex) are not UV resistant. If the material is
(European Group of FEF manufacturers). Sampling, subject to UV-rays it should be protected accordingly.
testing and evaluation were performed according to
CEN TS 16516, AgBB, ISO 16000-3, ISO 16000-6, 2.15 Re-use phase
ISO 16000-9, ISO 16000-11 in the latest versions. If removed properly the product can be re-used.
Based on the loading factor 0.05 m²/m³, which was Correctly sorted material can be ground and used to
determined after consideration of real life applications manufacture new products (e.g. ArmaSound).
with FEF products (in living rooms) and
recommendation of experts of the test institute, all 2.16 Disposal
results were clearly below the limit values. For Dispose of the materials according to local regulations.
example, the determined total volatile organic Regulated by the European Waste Catalogue: Waste
compound (TVOC) after 28 days was for all samples code 07 02 13 (waste plastic).
below 100 mg/m3. Certificates are available on Note: Please observe Commission Decision
request. 2001/118/EC.
2.17 Further information
2.13 Reference service life Further information on ArmaFlex® can be found on the
ArmaFlex products are long-lasting products. Findings manufacturer’s website www.armacell.com. Detailed
show that when used and installed properly they can specification clauses for the products are provided at
have an estimated service life of more than 50 years. www.armaflex.de.
4 Environmental Product Declaration Armacell GmbH – NH/ArmaFlex insulation for industrial and building installation
3. LCA: Calculation rules
3.1 Declared Unit country, the transport distance varies from 500 km to
The declaration refers to 1 m³ insulation product. 800 km
For the LCA calculations the average density per End-of-life (C2, C3):
product brand is used. The transport from place of usage to a waste
As additional information and support for installers the incineration plant is assumed as 100 km.
thermal conductivity coefficient (lambda-value) and R- After the demolition of the product a current realistic
value per 20 cm thickness per product brand are given. End-of-life scenario is the incineration of the material.
According to the reported net calorific value of the
Declared unit materials and the elementary composition, a partial
Name Value Unit stream consideration for the incineration process of
Declared unit 1 m3 PVC-products is applied as an approximation for all
Gross density 62.5 kg/m3 declared products.
Conversion factor to 1 kg 62.5 - Inventory estimations and approximations:
The reported recipes for the rubber mixes contain
Thermal conductivity λ : 0.040 W/(mK (0°C) specific substances of the rubber industry. For these
R-value – thickness: 20 cm: 5.0 (m²K)/W materials only partly life cycle inventories are available.
Approximations are used with the consideration of
similar supply chain effort or similar elementary
composition. Partly an estimation is modelled using
3.2 System boundary pre-products of the specific material and adding an
The data collection refers to the yearly production in energy effort as well as considering the treatment of
2019. The following life cycle stages are considered: production residues for this step in the supply chain.
Type of EPD: Cradle-to-Gate with options: 3.4 Cut-off criteria
In the assessment, all reported data from the
Production A1-A3: production process are considered, utilised thermal
The LCA calculation covers the production of the raw energy, and electric power consumption using best
materials (supply chain – A1), the mixing of raw available life cycle inventory (LCI) datasets. Thus
materials according to the respective recipes material and energy flows contributing less than 1% of
(MasterBatch) exclusively done in Münster, Germany, mass or energy are considered.
the transport (A2) of the MasterBatches to the No cut-off criteria are applied in the foreground data in
production facility for foaming and the foaming process this study.
(A3) in Germany, Spain, Poland or Great Britain, For cut-off criteria in the background system, see the
including the packaging material. information provided in the modelling principles and
Transport A4: specific documentations (documentation.gabi-
Average values for the transport from factory gate to software.com).
construction site are assumed.
Installation A5: 3.5 Background data
The installation considers the production of off-cuts, The LCA model is created using the GaBi ts Software
incineration of these off-cuts and the disposal scenario system (v9) for life cycle engineering, developed by
for the packaging material. Auxiliaries like adhesives or Sphera. The GaBi LCI database provides the life cycle
tapes or energy for installation are not considered. inventory data for several of the raw and process
End-of-life C2, C3: materials obtained from the background system. The
An incineration scenario for the used and demolished most recent update of the database was 2020 (service
product, including an assumption for the transport to pack 40).
disposal, is covered.
Benefits for the next product system D: 3.6 Data quality
Credits for electrical and thermal energy resulting from The foreground data collected by the manufacturer are
the waste incineration process of the off-cut material based on yearly production amounts and
and packaging (A5) and the product (C3) are declared extrapolations of measurements on specific machines
in module D. and plants.
Most of the necessary life cycle inventories for the
basic materials are available in the GaBi database.
The last update of the database was in 2020.
Further LCIs for materials of the supply chain of the
3.3 Estimates and assumptions basic materials are approximated with LCIs of similar
Scenario assumptions: materials or estimated by the combination of available
Installation (A5): LCIs.
The additional demand of material for installation For electrical and thermal energy regional specific grid
depends on the specific frame conditions of the mixes and regional specific supply for natural gas are
building and pipe system to be insulated. Parts of the considered.
product can be joined; thus installation off-cut is very
small. A loss of 1% is assumed. 3.7 Period under review
Transport to customer (A4): The production data refer to an average of the year
Armacell’s data collectors reported average figures for 2019.
the distribution of their material. Depending on the
5 Environmental Product Declaration Armacell GmbH – NH/ArmaFlex insulation for industrial and building installation
3.8 Allocation incinerated material. For the waste incineration plant
Allocation of upstream data: an R1-value of > 0.6 is assumed.
For all refinery products, allocation by mass and net Environmental burden of the incineration of installation
calorific value is applied. The specific manufacturing residues (off-cuts), packaging and the product in the
route of every refinery product is modelled and so the end-of-life scenario are assigned to the system (A5 or
impacts associated with the production of these C3); resulting credits for thermal and electrical energy
products are calculated individually. are declared in module D.
Materials and chemicals used in the manufacturing The credits for thermal and electrical energy are
process are modelled using the allocation rule most calculated via inversion of the life cycle inventory of
suitable for the respective product. For further European average data.
information on a specific product see Allocation for waste paper:
documentation.gabi-software.com. Paper/corrugated board is used as packaging material
Allocation in the foreground data: and this usually includes a mix of recycled and virgin
Part of the production residues (ca. 2%) are used for fibres. When modelling the production of paper, the
the manufacturing of a non-declared product scrap paper that is used in this process has been
(ArmaSound). These materials leave the process assumed to be burden free. Similarly, waste paper
without further consideration of any treatment and arising in the product life cycle is assumed to be
without credit (cut-off-approach). recycled. Robust data on paper and cardboard
No further allocation is applied in the software model. recycling are not promptly available and refer to a very
The overall production of the Armacell production complex system. Hence, to apply this methodology
facilities comprises further products beside the consistently throughout the model, a cut-off approach
products considered in this study. Data for thermal and has been applied, i.e., input of waste paper is
electrical energy, as well as auxiliary material, refer to considered without environmental burden, resulting
the declared products only. During data collection the waste paper is not credited. The recycling process and
allocation is done via mass, area, pieces or time spent the production process of paper are merged in the
in the machine, depending on the process step and production process. The C-balance referring to fresh
reasonable split. The data collectors at Armacell fibre is corrected via CO2 emissions (biotic)
decided on the distribution basis. (assumption of final rotting or incineration in the time
Allocation for waste materials: frame of 100 years).
Production waste is sent to a waste incineration plant
and to landfill (Spain). Resulting electrical and thermal 3.9 Comparability
energy from the incineration process is looped inside Basically, a comparison or an evaluation of EPD data
module A1-A3. The quality of the recovered energy is is only possible if all the data sets to be compared
assumed to the same as that of the input energy. were created according to EN 15804 and the building
Landfilling of plastic material is assumed not to deliver context, respectively the product-specific
any landfill gas. characteristics of performance, are taken into account.
All applied incineration processes are displayed via a
partial stream consideration for the combustion The used background dataset DB has been GaBi
process, according to the specific composition of the (service pack 40, 2020).
4. LCA: Scenarios and additional technical information
Characteristic product properties
Information on biogenic Carbon Transport to the building site (A4)
The biogenic carbon content quantifies the amount of Name Value Unit
biogenic carbon in a construction product leaving the Litres of fuel 0.2 l/100km
factory gate, and it shall be separately declared for the Transport distance 800 km
product and any accompanying packaging.If the total Capacity utilisation (including empty
85 %
mass of biogenic carbon containing materials is less runs)
than 5 % of the total mass of the product and
accompanying packaging, the declaration of biogenic Installation into the building (A5)
carbon content may be omitted. The mass of Name Value Unit
packaging containing biogenic carbon shall always be Material loss 1 %
declared.Note: 1 kg biogenic Carbon is equivalent to
44/12 kg of CO2
Information on describing the biogenic Carbon Estimated service life
Content at factory gate Name Value Unit
Name Value Unit Life Span according to the
50 a
Biogenic Carbon Content in manufacturer
0 kg C
product
Biogenic Carbon Content in End of life (C1-C4)
26.93 kg C
accompanying packaging Name Value Unit
The embodied biogenic carbon leaves the system in Energy recovery in WIP 62,5 kg
Module A5.
Reuse, recovery and/or recycling potentials (D),
relevant scenario information
The following technical information serves as a basis Module D includes the credits of the incineration
for the declared modules. The values refer to the processes from A5 (off-cut of product installation,
declared unit of 1 m³. packaging waste) and C3 (incineration of the product).
6 Environmental Product Declaration Armacell GmbH – NH/ArmaFlex insulation for industrial and building installation
A waste incineration plant with an R1-value > 0.6 is
assumed.
7 Environmental Product Declaration Armacell GmbH – NH/ArmaFlex insulation for industrial and building installation
5. LCA: Results
The following information on environmental impacts is expressed with the impact category parameters of LCIA
using characterisation factors. The chosen characterisation factors fulfil the requirements of EN 15804.
Disclaimer:
EP-freshwater: This indicator has been calculated as “kg P eq” as required in the characterization model
(EUTREND model, Struijs et al., 2009b, as implemented in ReCiPe;
http://eplca.jrc.ec.europa.eu/LCDN/developerEF.xhtml)
DESCRIPTION OF THE SYSTEM BOUNDARY (X = INCLUDED IN LCA; ND = MODULE OR INDICATOR NOT
DECLARED; MNR = MODULE NOT RELEVANT)
BENEFITS AND
CONSTRUCTI LOADS
PRODUCT STAGE ON PROCESS USE STAGE END OF LIFE STAGE BEYOND THE
STAGE SYSTEM
BOUNDARIES
8 Environmental Product Declaration Armacell GmbH – NH/ArmaFlex insulation for industrial and building installation
lairetam
waR
ylppus tropsnarT
gnirutcafunaM
eht
morf
tropsnarT
etis
eht
ot
etag
ylbmessA esU
ecnanetniaM
riapeR
tnemecalpeR tnemhsibrufeR
ygrene
lanoitarepO esu
retaw
lanoitarepO esu
noitcurtsnoc-eD
noitilomed tropsnarT
gnissecorp
etsaW
lasopsiD -esueR -yrevoceR -gnilcyceR laitnetop
A1 A2 A3 A4 A5 B1 B2 B3 B4 B5 B6 B7 C1 C2 C3 C4 D
X X X X X ND ND MNR MNR MNR ND ND ND X X ND X
RESULTS OF THE LCA - ENVIRONMENTAL IMPACT according to EN 15804+A2: 1 m³ NH/ArmaFlex
insulation for industrial and building installation
Core Indicator Unit A1-A3 A4 A5 C2 C3 D
Global warming potential - total [kg CO2-Eq.] 2.17E+2 4.83E+0 1.09E+2 2.98E-1 1.62E+2 -4.61E+1
Global warming potential - fossil fuels [kg CO2-Eq.] 3.16E+2 4.79E+0 5.69E+0 2.96E-1 1.62E+2 -4.59E+1
Global warming potential - biogenic [kg CO2-Eq.] -9.91E+1 -8.19E-3 1.03E+2 -5.06E-4 -7.08E-2 -1.08E-1
GWP from land use and land use change [kg CO2-Eq.] 8.54E-1 3.88E-2 9.55E-3 2.40E-3 3.30E-2 -3.21E-2
Depletion potential of the stratospheric ozone layer [kg CFC11-Eq.] 7.45E-10 5.76E-16 7.53E-12 3.56E-17 2.47E-13 -4.78E-13
Acidification potential, accumulated exceedance [mol H+-Eq.] 5.50E-1 1.44E-2 9.00E-3 8.88E-4 4.82E-2 -6.42E-2
Eutrophication, fraction of nutrients reaching freshwater
end compartment
[kg PO4-Eq.] 2.50E-3 1.46E-5 2.62E-5 9.01E-7 4.16E-5 -5.90E-5
Eutrophication, fraction of nutrients reaching marine end
[kg N-Eq.] 2.01E-1 6.40E-3 3.17E-3 3.95E-4 1.59E-2 -1.66E-2
compartment
Eutrophication, accumulated exceedance [mol N-Eq.] 1.90E+0 7.17E-2 3.52E-2 4.43E-3 1.95E-1 -1.78E-1
Formation potential of tropospheric ozone photochemical
[kg NMVOC-Eq.] 6.63E-1 1.26E-2 9.76E-3 7.81E-4 4.51E-2 -4.78E-2
oxidants
Abiotic depletion potential for non-fossil resources [kg Sb-Eq.] 5.17E+3 6.38E+1 6.02E+1 3.94E+0 2.99E+2 -7.79E+2
Abiotic depletion potential for fossil resources [MJ] 6.99E-4 3.44E-7 7.13E-6 2.12E-8 3.55E-6 -7.52E-6
Water (user) deprivation potential, deprivation-weighted [m³ world-Eq
1.95E+1 4.29E-2 2.36E+0 2.65E-3 1.25E+1 -4.74E+0
water consumption (WDP) deprived]
RESULTS OF THE LCA - INDICATORS TO DESCRIBE RESOURCE USE according to EN 15804+A2: 1 m³
NH/ArmaFlex insulation for industrial and building installation
Indicator Unit A1-A3 A4 A5 C2 C3 D
Renewable primary energy as energy carrier [MJ] 1.99E+3 3.59E+0 1.60E+2 2.22E-1 6.20E+1 -1.70E+2
Renewable primary energy resources as material utilization [MJ] 1.37E+2 0.00E+0 -1.37E+2 0.00E+0 0.00E+0 0.00E+0
Total use of renewable primary energy resources [MJ] 2.13E+3 3.59E+0 2.29E+1 2.22E-1 6.20E+1 -1.70E+2
Non-renewable primary energy as energy carrier [MJ] 4.14E+3 6.39E+1 6.93E+1 3.95E+0 1.32E+3 -7.79E+2
Non-renewable primary energy as material utilization [MJ] 1.03E+3 0.00E+0 -9.13E+0 0.00E+0 -1.03E+3 0.00E+0
Total use of non-renewable primary energy resources [MJ] 5.17E+3 6.39E+1 6.02E+1 3.95E+0 2.99E+2 -7.79E+2
Use of secondary material [kg] 3.83E+1 0.00E+0 0.00E+0 0.00E+0 0.00E+0 0.00E+0
Use of renewable secondary fuels [MJ] 0.00E+0 0.00E+0 0.00E+0 0.00E+0 0.00E+0 0.00E+0
Use of non-renewable secondary fuels [MJ] 0.00E+0 0.00E+0 0.00E+0 0.00E+0 0.00E+0 0.00E+0
Use of net fresh water [m³] 1.47E+0 4.15E-3 6.61E-2 2.57E-4 3.29E-1 -1.96E-1
RESULTS OF THE LCA – WASTE CATEGORIES AND OUTPUT FLOWS according to EN 15804+A2:
1 m³ NH/ArmaFlex insulation for industrial and building installation
Indicator Unit A1-A3 A4 A5 C2 C3 D
Hazardous waste disposed [kg] 2.88E-5 2.97E-6 3.38E-7 1.84E-7 1.35E-6 -3.11E-7
Non-hazardous waste disposed [kg] 3.55E+1 9.78E-3 1.54E+0 6.04E-4 9.94E+1 -3.59E-1
Radioactive waste disposed [kg] 1.11E-1 7.91E-5 1.46E-3 4.89E-6 9.49E-3 -5.79E-2
Components for re-use [kg] 0.00E+0 0.00E+0 0.00E+0 0.00E+0 0.00E+0 0.00E+0
Materials for recycling [kg] 0.00E+0 0.00E+0 5.38E+1 0.00E+0 0.00E+0 0.00E+0
Materials for energy recovery [kg] 0.00E+0 0.00E+0 0.00E+0 0.00E+0 0.00E+0 0.00E+0
Exported electrical energy [MJ] 0.00E+0 0.00E+0 2.88E+1 0.00E+0 1.63E+2 0.00E+0
Exported thermal energy [MJ] 0.00E+0 0.00E+0 5.17E+1 0.00E+0 2.98E+2 0.00E+0
RESULTS OF THE LCA – additional impact categories according to EN 15804+A2-optional:
1 m³ NH/ArmaFlex insulation for industrial and building installation
Indicator Unit A1-A3 A4 A5 C2 C3 D
Potential incidence of disease due to PM emissions [Disease
6.72E-6 7.96E-8 9.51E-8 4.92E-9 1.16E-6 -5.45E-7
Incidence]
Potential Human exposure efficiency relative to U235 [kBq U235-
1.04E+1 1.14E-2 1.53E-1 7.07E-4 9.63E-1 -9.50E+0
Eq.]
Potential comparative toxic unit for ecosystems [CTUe] 4.49E+3 4.51E+1 5.02E+1 2.79E+0 2.48E+2 -1.68E+2
Potential comparative toxic unit for humans - cancerogenic [CTUh] 7.48E-8 9.45E-10 9.90E-10 5.84E-11 9.80E-9 -7.28E-9
Potential comparative toxic unit for humans - not cancerogenic [CTUh] 5.49E-6 5.49E-8 7.15E-8 3.40E-9 1.04E-6 -2.70E-7
Potential soil quality index [-] 6.36E+3 2.24E+1 6.63E+1 1.38E+0 6.78E+1 -1.22E+2
Disclaimer 1 – for the indicator IRP
This impact category deals mainly with the eventual impact of low dose ionizingradiation on human health of the
nuclear fuel cycle. It does not consider effects due to possiblenuclear accidents, occupational exposure nor due to
radioactive waste disposal in undergroundfacilities. Potential ionizing radiation from the soil, from radon and some
construction materials is also not measured by this indicator.
Disclaimer 2 – for the indicators ADPE, ADPF, WDP, ETP-fw, HTP-c, HTP-nc, SQP
The results of this environmental impact indicator shall be used with care as theuncertainties on these results are
high or as there is limited experience with the indicator.
6. LCA: Interpretation
The supply chain, i.e. the production of the purchased the overall green house gas emissions. At the same
materials, causes the highest influence on all impact time a credit (D) of 10% is given to the next system,
categories and the primary energy. due to the use of electrical and thermal energy, gained
in the incineration processes for the product and the
Global Warming Potential off-cut material.
Looking at the GWP for the overall declared life cycle
phases, including production (A1-A3), transport (A4, Further impact categories
C2), installation (losses) (A5) and end-of-life (C3, D), The end-of-life scenarios have less influence on the
the production (A1-A3) contributes to 49%. other considered impact categories than on GWP. The
The production in the supply chain (A1) already main contribution of the considered life cycle phases is
contributes 40% to the total GWP value. Thus, every concentrated on module A1-A3.
increase in the production yield directly improves the The energy consumption in the foaming step
environmental performance of the products. influences all impact categories; variations depend on
The foaming process (A3), which includes the the national grid mixes for electricity.
electrical and thermal energy for the mixing, the
vulcanisation and blowing step as well as the Primary Energy Demand
production of the packaging materials, shows a The total primary energy demand is for both categories
significant influence on GWP of the life cycle with 9%. (renewable and non-renewable) significantly (> 100%)
Module A5 covers the production and disposal influenced by the production of the module A1-A3. The
(=incineration) of the off-cut material assumed as 1% other modules play a minor role (C3 with about 5%)
loss in respect to the required insulation material.
Additionally, the emissions of the incineration of The share of primary energy bound as material
packaging material (plastic, wood) in a waste accounts for about 17%, which is partly recovered and
incineration plant are considered. The installation step credited for in module D (-14%)
contributes with 24% to the overall GWP.
As end-of-life scenario an incineration is considered.
The emissions of the product (C3) contribute to 36% to
7. Requisite evidence
recommendation of the experts of the test institute, all
7.1 VOC emissions results were clearly below the limit values. For
Eurofins Product Testing A/S has tested a wide range example the determined total volatile organic
and varieties of typical FEF (Flexible Elastomeric compound (TVOC) after 28 days was for all samples
Foam) products marketed in the EU from CEFEP below 100 mg/m3. Certificates are available on
(European Group of FEF manufacturers). Sampling, request.
testing and evaluation were performed according to
CEN TS 16516, AgBB, ISO 16000-3, ISO 16000-6, 7.2 Leaching performance
ISO 16000-9, ISO 16000-11 in the latest versions. According to EN 13468 is the content of water-soluble
Based on the loading factor 0.05 m²/m³, which were chloride ions for NH/Armaflex ≤ 80 ppm.
determined after consideration of real life applications
with FEF products (in living rooms) and
8. References
9 Environmental Product Declaration Armacell GmbH – NH/ArmaFlex insulation for industrial and building installation
AgBB EN 14707
Umweltbundesamt Germany, Health-related EN 14707: 2013-01: Thermal insulating products for
Evaluation of Emissions of Volatile Organic building equipment and industrial installations -
Compounds (VVOC, VOC and SVOC) from Building Determination of maximum service temperature for
Products preformed pipe insulation
CEFEP EN 15801
The industry association for FEF and PEF insulation EN 15801: 2010-04: Conservation of cultural property -
(Celle) in 2012 Test methods - Determination of water absorption by
capillarity
CEN TS 16516
CEN TS 16516:2013-12: Construction products - EN 15804
Assessment of release of dangerous substances - EN 15804:2012-04+A1 2013, Sustainability of
Determination of emissions into indoor air construction works — Environmental Product
Declarations — Core rules for the product category of
Comission Decision 2001/118/EC construction products.
Amendment to European Waste Catalogue
EN 15804
CPR EN 15804:2019+A2 (in press), Sustainability of
Regulation (EC) No 305/2011, Construction Products construction works — Environmental Product
Regulation Declarations — Core rules for the product category of
construction products.
EN 826
EN 826: 2013-05: Thermal insulating products for EN 29052
building applications - Determination of compression EN 29052: 1992-08: Acoustics; determination of
behaviour dynamic stiffness; part 1: materials used under floating
floors in dwellings
EN 1606
EN 1606: 2013-05: Thermal insulating products for EU/EFTA
building applications - Determination of compressive Regulation (EU) No. 305/2011 (CPR), European
creep Union/European Free Trade Association (EU/EFTA)
EN 12091 Eurofins Product Testing A/S
EN 12091: 2013-06: Thermal insulating products for Eurofins Miljo, Smedeskowej 38, 8464 Galten,
building applications - Determination of freeze-thaw Denmark
resistance
European Waste Catalogue
EN 12086 European Waste Catalogue and Hazardous Waste
EN 12086:2013-06: Thermal insulating products for List, Commission Decision 2000/532/EC
building applications - Determination of water vapour
transmission properties GaBi
GaBi 9 software-system and databases, LBP,
EN 13468 University of Stuttgart and Sphera, Leinfelden-
EN 13468: 2001-12: Thermal insulating products for Echterdingen, 2020 (http://documentation.gabi-
building equipment and industrial installations - software.com/)
Determination of trace quantities of water soluble
chloride, fluoride, silicate, and sodium ions and pH IBU
Institut Bauen und Umwelt e.V.: General Programme
EN 13469 Instructions for the Preparation of EPDs at the Institut
EN 13469:2013-01: Thermal insulating products for Bauen und Umwelt e.V. Version 1., Berlin: Institut
building equipment and industrial installations - Bauen und Umwelt e.V., 2016. www.ibu-epd.com
Determination of water vapour transmission properties
of preformed pipe insulation IBU PCR Part A
PCR - Part A: Calculation Rules for the Life Cycle
EN 13501-1 Assessment and Requirements on the Project Report,
EN 13501-1: 2010-01: Fire classification of Institut Bauen und Umwelt e.V., www.ibu-epd.com,
construction products and building elements - Part 1: 2019.
Classification using data from reaction to fire tests
IBU PCR PART B
EN 14304 PCR – Part B: Requirements on the EPD for Insulation
EN 14304:2013-04: Thermal insulation products for materials made of foam plastics, version 1.7, 01-2019 ,
building equipment and industrial installations – Institut Bauen und Umwelt e.V., www.ibu-epd.com,
Factory made flexible elastomeric foam (FEF) products 2019
– Specification
ISO 3822-1
EN 14706 ISO 3822-1: 1999-05: Acoustics - Laboratory tests on
EN 14706: 2013-01: Thermal insulating products for noise emission from appliances and equipment used in
building equipment and industrial installations - water supply installations - Part 1: Method of
Determination of maximum service temperature measurement
10 Environmental Product Declaration Armacell GmbH – NH/ArmaFlex insulation for industrial and building installation
ISO 9001 Sampling, storage of samples and preparation of test
ISO 9001:2014-08: Quality management systems – specimens
Requirements
ISO 16000-3
ISO 11654 ISO 16000-3:2011-10: Determination of formaldehyde
ISO 11654: 1997-04: Acoustics - Sound absorbers for and other carbonyl compounds in indoor air and test
use in buildings - Rating of sound absorption chamber air - Active sampling method
ISO 14001 ISO 16000-6
ISO 14001:2015, Environmental management systems ISO 16000-6:2011-12: Indoor air - Part 6:
— Requirements with guidance for use Determination of volatile organic compounds in indoor
and test chamber air by active sampling on Tenax TA®
ISO 14025 sorbent, thermal desorption and gas chromatography
ISO 14025:2011-10, Environmental labels and using MS or MS-FID
declarations — Type III environmental declarations —
Principles and procedures. ISO 16000-9
ISO 16000-9:2006-02: Indoor air - Part 9:
ISO 14040 Determination of the emission of volatile organic
ISO 14040:2009-11: Environmental management – compounds from building products and furnishing -
Life cycle assessment – Principles and framework Emission test chamber method
ISO 14044
ISO 14044:2006-10: Environmental management – REACH
Life cycle assessment – Requirements and guidelines Regulation (EC) No 1907/2006, Regulation concerning
the Registration, Evaluation, Authorisation and
ISO 15868 Restriction of Chemicals (REACH)
ISO 15686:2011-05, Buildings and constructed assets
- Service life planning
ISO 16000-11
ISO 16000-11: 2006-02: Indoor air - Part 11:
Determination of the emission of volatile organic
compounds from building products and furnishing -
11 Environmental Product Declaration Armacell GmbH – NH/ArmaFlex insulation for industrial and building installation
Publisher
Institut Bauen und Umwelt e.V. Tel +49 (0)30 3087748- 0
Panoramastr. 1 Fax +49 (0)30 3087748- 29
10178 Berlin Mail info@ibu-epd.com
Germany Web www.ibu-epd.com
Programme holder
Institut Bauen und Umwelt e.V. Tel +49 (0)30 - 3087748- 0
Panoramastr 1 Fax +49 (0)30 – 3087748 - 29
10178 Berlin Mail info@ibu-epd.com
Germany Web www.ibu-epd.com
Author of the Life Cycle
Assessment Tel +49 711 341817-0
Sphera Solutions GmbH Fax +49 711 341817-25
Hauptstraße 111- 113 Mail info@sphera.com
70771 Leinfelden-Echterdingen Web http://www.sphera.com
Germany
Owner of the Declaration
Armacell GmbH Tel +49-251-7603-0
Robert-Bosch-Str. 10 Fax +49-251-7603-346
48153 Münster Mail info.de@armacell.com
Germany Web www.armacell.de
