ENVIRONMENTAL PRODUCT DECLARATION
as per ISO 14025 and EN 15804+A1
Owner of the Declaration ArcelorMittal Brasil
Programme holder Institut Bauen und Umwelt e.V. (IBU)
Publisher Institut Bauen und Umwelt e.V. (IBU)
Declaration number EPD-ARM-20210054-CBC1-EN
ECO EPD Ref. No.
Issue date 26.07.2021
Valid to 25.07.2026
Reinforcing steel in bars
ArcelorMittal Brasil
www.ibu-epd.com | https://epd-online.com
Umwelt Produktdeklaration Name des Herstellers – Name des Produkts
General Information
ArcelorMittal Brasil Reinforcing steel in bars
Programme holder Owner of the declaration
IBU – Institut Bauen und Umwelt e.V. ArcelorMittal Brasil
Panoramastr. 1 Avenida Carandaí, 1115
10178 Berlin Funcionários - 16o andar
Germany 30130-915 - Belo Horizonte
Brasil
Declaration number Declared product / declared unit
EPD-ARM-20210054-CBC1-EN 1 metric ton of reinforcing steel bars produced by
ArcelorMittal in Brazil
This declaration is based on the product Scope:
category rules: The declaration applies to 1 metric ton of reinforcing
Reinforcing Steel, 30.11.2017 steel bar produced by ArcelorMittal Brasil, representing
(PCR checked and approved by the SVR) 100% of the annual production of 2019.
Issue date The owner of the declaration shall be liable for the
26.07.2021 underlying information and evidence; the IBU shall not
be liable with respect to manufacturer information, life
cycle assessment data and evidences.
Valid to
The EPD was created according to the specifications
25.07.2026
of EN 15804+A1. In the following, the standard will be
simplified as EN 15804.
Verification
The standard EN 15804 serves as the core PCR
Independent verification of the declaration and data
according to ISO 14025:2010
Dipl. Ing. Hans Peters internally x externally
(chairman of Institut Bauen und Umwelt e.V.)
Dr. Alexander Röder Dr. Eva Schmincke
(Managing Director Institut Bauen und Umwelt e.V.)) (Independent verifier)
Product
Information about the enterprise  NB 732
ArcelorMittal is the world’s leading steel and mining  NTP 339
company. Guided by a philosophy to produce safe,
 NTP 341
sustainable steel, it is the leading supplier of quality
 NCh 204
steel products in all major markets including
automotive, construction, household appliances and  NTC 2289
packaging. ArcelorMittal is present in 60 countries.  IRAM 500-207
 IRAM 500-528
Product description/Product definition
 PNA 4-007-99
Rebar is short for reinforcing (steel) bar, used for the
reinforcement of concrete according to EN10080  FONDONORMA 316
standard (as weldable reinforcing steel in bars and  ASTM A615
coils).  ASTM A706
For the use and application of the product, the
respective national provisions at the place of use
Application
apply, being
Reinforcing steel bars (rebar) are steel rods that are
 ABNT NBR 6118
used as a tension device in concrete. Typical
 ABNT NBR 6215
applications are in the construction of buildings,
 ABNT NBR 7477 bridges, roads and other civil works (infrastructure,
 ABNT NBR 7478 superstructures etc.).
 ABNT NBR 7480
 ISO 6892
 ISO 15630
2 Environmental Product Declaration ArcelorMittal – Reinforcing steel in bars
 Pig iron and scrap are converted into steel in
an electric arc furnace;
Technical Data
 Produced steel refined in a ladle furnace with
Technical specifications are listed below.
addition of ferroalloys and metals to obtain
Constructional data the required steel characteristics;
Rebar can be produced either by an Electric Arc  Steel is then casted at a continuous caster
Furnace (EAF) of a Basic Oxygen Furnace (BOF) and then rolled to obtain the rebars.
route.
Name Value Unit
The first step is either performed internally or by
Tensile strength (CA25) 30 N/mm2
external suppliers.
Tensile strengh (CA50/AP 500/AH 540/550/60
N/mm^2
500) 0
Environment, Health and Safety (EHS)
Type of steel (Bar, coil, welded
- -
fabric, lattice grinders)
Environmental, occupational health, safety and quality
Production route (EAF or BOF) - -
management at the different plants of ArcelorMittal in
Weldability (max) 0.55 Ceq
Brasil are in accordance with the following standards:
Yield strength (CA25) 250 N/mm2
 ISO 14001;
Yield strength (CA50/AP 500/AH
500 N/mm^2  ISO 45001;
500)
Surface geometry (fR or PRA)  Environmental labelling – Type I, provided by
Flat -
(CA25) the Associação Brasileira de Normas
Surface geometry (fR or PRA) Técnicas – ABNT (Brazilian National
Rib
(CA50/AP 500/AH 500) Standards Organization), developed
Elongation (Agt) (CA25) 18 % according to the standards ISO 14020 and
Elongation (Agt) (CA50/AP
8 % ISO 14024.
500/AH 500)
End of life scenario - Re-use phase
Performance data of the product with respect to its
characteristics in accordance with the relevant Deconstruction
technical provision (no CE-marking).
Reinforcing steel bars (rebar) are not reused at the end
Base materials/Ancillary materials of life but can be easily separated from the concrete
The base material for the rebar is iron. Alloying and recycled into similar steel products.
elements are added in the form of ferroalloys or metal,
the most common elements are manganese, Recycling and recovery
chromium and vanadium. Other elements like copper
may be present in steel. Reinforcing steel bar (rebar) is 100% recyclable and
can be recycled to the same (or higher/lower) quality of
This product/article/at least one partial article contains steel depending upon the metallurgy and processing of
substances listed in the candidate list (date: the recycling route. Recycling routes are well
27.06.2018) exceeding 0.1 percentage by mass: no” established in Brasil and recycling should be preferred
(as) at end of life.
Maximum content on the following elements are
established by the Brazilian National Standard ABNT The efficiency of the recycling process is 85%
NBR 7480: (ArcelorMittal 2016). Reuse, Recovery and Recycling
 % Carbon: 0,35 maximum; potential of this fraction of rebar is reported in module
D.
 % Manganese: 1,50 maximum;
 % Phosphorus: 0,050 maximum;
Disposal
 % Sulphur: 0,050 maximum;
 % Silicon: 0,50 maximum. Reinforcing steel bars (rebar) is a valuable resource
and therefore should not be disposed. ArcelorMittal
has scrap yards and partners working all over Brazil to
The standard ABNT NBR 7480, also allows for
enable scrap collection and to provide logistic support.
ferroalloy content of elements like niobium, vanadium,
but with a Carbon Equivalent Value (CEV) not
The fraction of steel scraps that cannot be recovered
exceeding 0,55% analysis in the ladle furnace,
(due to collection loss) is landfilled. The Brazilian
according the following equation:
Waste Index for iron and steel is 17 04 05.
CE=C+Mn/6+ (Cr+V+Mo)/5+ (Cu+Ni)/15
Reference service life
Manufacture
As rebar is used in concrete structures to give
additional mechanical resistance, its lifetime will be
In ArcelorMittal Brasil rebars are produced by the
limited by the service life of the building.
following process steps:
 Iron ore and charcoal are fed to a blast
The documentation of the RSL, under this
furnace to produce pig iron; circumstance, is not required for the current EPD
3 Environmental Product Declaration ArcelorMittal – Reinforcing steel in bars
according to the relevant ISO standards and EN  https://brasil.arcelormittal.com.br/produtos-
15804. solucoes/construcao-civil/vergalhao-
arcelormittal-ca-50-s-soldavel
Additional information
Additional information on reinforcing steel bars (rebar)
can be found at:
 https://brasil.arcelormittal.com/produtos-
solucoes/catalogos
LCA: Calculation rules
Declared Unit  Transport of resources and additives to the
production site
The declared unit is 1 metric tonne of reinforcing steel
 Production processes on-site including
bars, packed and ready to be transported from
energy, production of additives, disposal of
ArcelorMittal Brasil to their clients as specified in Part
B: Requirements on the EPD for Structural Steel, production residues, and consideration of
Institut Bauen und Umwelt e.V (PCR 2017, Part B). related emissions
 Recycling of production/manufacturing scrap.
Declared unit Steel scrap is assumed to reach the end-of-
Name Value Unit
waste status once it is shredded and sorted,
Declared unit 1 t
thus becomes the input to the product system
Density 7825 kg/m3
in the inventory.
Conversion factor to 1 kg 0.001 -
The data for the life cycle inventory are based on data Module C3 takes into account the sorting and
covering 100% of the production volume of rebar in shredding of after-use steel that is recycled, as well as
Brazil in 2019. the non-recovered scrap due to sorting efficiency
which is landfilled. A conservative value of 1% landfill
All reported data are calculated as total value per site is considered.
averaged across all production sites based on
production volume per site. Module D refers to the end-of-life of hot-dip coated
steel wire, including reuse and recycling. For recycling,
the net amount of steel scrap made available over the
System boundary whole life cycle is considered.
The of the EPD: cradle-to-gate with options. Module Comparability
A1-A3, Module C3 and Module D were considered. Basically, a comparison or an evaluation of EPD data
is only possible if all the data sets to be compared
Modules A1-A3 of hot-dip coated steel wire production were created according to EN 15804 and the building
include the following: context, respectively the product-specific
 The provision of resources, additives, and characteristics of performance, are taken into account.
energy
The background database used for this EPD is GaBi,
SP 30..
LCA: Scenarios and additional technical information
Reuse, recovery and/or recycling potentials (D),
relevant scenario information
Module D includes any declared benefits and loads
End of life (C1 - C4) from net flows leaving the product system that have
not been allocated as co-products and that have
This module considers the scrap preparation after passed the end-of-waste state in the form of recovery
initial sorting and shredding of the end-of-life steel, as and/or recycling potentials.
well as the non-recovered scrap due to sorting
efficiency, which ends up in landfills. The end-of-life The benefits brought by the 85% recycling rate of
scenario for concrete steel bars considers that after scrap is applied to the net output leaving the product
use 15% is landfilled. system since it becomes an avoided production of
virgin material.
Name Value Unit Name Value Unit
Landfilling 150 kg Recycling 850 kg
4 Environmental Product Declaration ArcelorMittal – Reinforcing steel in bars
LCA: Results
DESCRIPTION OF THE SYSTEM BOUNDARY (X = INCLUDED IN LCA; MND = MODULE NOT DECLARED;
MNR = MODULE NOT RELEVANT)
BENEFITS AND
CONSTRUCTI LOADS
PRODUCT STAGE ON PROCESS USE STAGE END OF LIFE STAGE BEYOND THE
STAGE SYSTEM
BOUNDARIES
5 Environmental Product Declaration ArcelorMittal – Reinforcing steel in bars
lairetam
waR
ylppus tropsnarT
gnirutcafunaM
eht
morf
tropsnarT
etis
eht
ot
etag
ylbmessA esU
ecnanetniaM
riapeR
tnemecalpeR tnemhsibrufeR
ygrene
lanoitarepO esu
retaw
lanoitarepO esu
noitcurtsnoc-eD
noitilomed tropsnarT
gnissecorp
etsaW
lasopsiD -esueR -yrevoceR -gnilcyceR laitnetop
A1 A2 A3 A4 A5 B1 B2 B3 B4 B5 B6 B7 C1 C2 C3 C4 D
X X X MND MND MND MND MNR MNR MNR MND MND MND MND X MND X
RESULTS OF THE LCA - ENVIRONMENTAL IMPACT according to EN 15804+A1: 1 metric to reinforcing
steel bars
Parameter Unit A1-A3 C3 D
Global warming potential [kg CO2-Eq.] 8.81E+2 3.43E+0 -4.82E+2
Depletion potential of the stratospheric ozone layer [kg CFC11-Eq.] 5.53E-8 6.26E-14 2.96E-12
Acidification potential of land and water [kg SO2-Eq.] 2.65E+0 2.08E-2 -1.11E+0
Eutrophication potential [kg (PO4)3--Eq.] 2.60E-1 2.24E-3 -9.23E-2
Formation potential of tropospheric ozone photochemical
[kg ethene-Eq.] 2.01E-1 1.64E-3 -1.45E-1
oxidants
Abiotic depletion potential for non-fossil resources [kg Sb-Eq.] 2.08E-4 4.41E-7 1.15E-5
Abiotic depletion potential for fossil resources [MJ] 5.95E+3 4.30E+1 -3.81E+3
RESULTS OF THE LCA - INDICATORS TO DESCRIBE RESOURCE USE according to EN 15804+A1: 1
metric to reinforcing steel bars
Parameter Unit A1-A3 C3 D
Renewable primary energy as energy carrier [MJ] 3.15E+3 2.11E+1 4.15E+2
Renewable primary energy resources as material utilization [MJ] 0.00E+0 0.00E+0 0.00E+0
Total use of renewable primary energy resources [MJ] 3.15E+3 2.11E+1 4.15E+2
Non-renewable primary energy as energy carrier [MJ] 6.25E+3 4.51E+1 -3.64E+3
Non-renewable primary energy as material utilization [MJ] 0.00E+0 0.00E+0 0.00E+0
Total use of non-renewable primary energy resources [MJ] 6.25E+3 4.51E+1 -3.64E+3
Use of secondary material [kg] 6.73E+2 0.00E+0 0.00E+0
Use of renewable secondary fuels [MJ] 6.51E-19 3.77E-19 0.00E+0
Use of non-renewable secondary fuels [MJ] 7.65E-18 4.43E-18 0.00E+0
Use of net fresh water [m³] 1.60E+1 9.60E-2 -3.28E-1
RESULTS OF THE LCA – WASTE CATEGORIES AND OUTPUT FLOWS according to EN 15804+A1:
1 metric to reinforcing steel bars
Parameter Unit A1-A3 C3 D
Hazardous waste disposed [kg] 5.99E-5 5.43E-7 -3.08E-6
Non-hazardous waste disposed [kg] 4.30E+0 1.50E+2 -6.93E+0
Radioactive waste disposed [kg] 1.14E-1 7.97E-4 6.61E-2
Components for re-use [kg] 0.00E+0 0.00E+0 0.00E+0
Materials for recycling [kg] 0.00E+0 8.50E+2 0.00E+0
Materials for energy recovery [kg] 0.00E+0 0.00E+0 0.00E+0
Exported electrical energy [MJ] 0.00E+0 0.00E+0 0.00E+0
Exported thermal energy [MJ] 0.00E+0 0.00E+0 0.00E+0
References
ABNT NBR 6118 ABNT NBR 7478
ABNT NBR 6118:2014 - Design of concrete structures ABNT NBR 7478:2021 - Fatigue test method of steel
— Procedure bars for reinforced concrete
ABNT NBR 6215 ABNT NBR 7480
ABNT NBR 6215:2011 - Steel products — Terminology ABNT NBR 7480:2007 - Steel for the reinforcement of
concrete structures – Specification
ABNT NBR 7477
ABNT NBR 7477:1982 - Determination of the surface Environmental labelling – Type I
conformation coefficient of steel bars and wires for Environmental labelling – Type I provided
reinforced concrete by Associação Brasileira de Normas Técnicas – ABNT
(Brazilian National Standards ISO 6892
Organization) http://www.abnt.org.br/ ISO 6892-1:2019 - Metallic materials — Tensile testing
— Part 1: Method of test at room temperature
ASTM A615
ASTM A615:2020 - Standard specification for ISO 14001
deformed and plain carbon-steel bars for concrete ISO 14001:2015 - Environmental management
reinforcement systems - Requirements with guidance for use
ASTM A706 ISO 14020
ASTM A706:2016 - Standard specification for ISO 14020:2000 - Environmental labels and
deformed and plain low-alloy steel Bars for concrete declarations — General principles
reinforcement
ISO 14024
Brazilian Waste Index ISO 14024:2018 - Environmental Labels and
Normative Instruction No. 1, of January 25, 2013, declarations - Type I environmental labelling -
regulates the National Register of Operators of Principles and Procedures
Hazardous Waste (CNORP)
http://www.ibama.gov.br/component/content/article?id= ISO 14025
726 EN ISO 14025:2011-10, Environmental labels and
declarations — Type III environmental declarations —
Candidate List of Substances of Very High Principles and procedures.
Concern of Authorization
Regulation (EC) No 1907/2006 of the European ISO 15630
Parliament and of the Council on the Registration, ISO 15630-1:2019 - Steel for the reinforcement and
Evaluation, Authorisation and Restriction of Chemicals prestressing of concrete — Test methods — Part 1:
(REACH) Reinforcing bars, rods and wire
https://echa.europa.eu/candidate-list-table
ISO 45001
EN10080 ISO 45001:2018 - Occupational health and safety
EN10080:2005 - Steel for the reinforcement of management systems ￿. Requirements with guidance
concrete - Weldable reinforcing steel – General for use
EN 15804 NB 732
EN 15804:2012-04+A1 2013: Sustainability of NB 732:2017 - Productos laminados - Barras
construction works — Environmental Product corrugadas para hormigón armado - Definiciones,
Declarations — Core rules for the product category of clasificación y requisitos
construction products
NCh 204
European Chemicals Agency NCh 204:2020 - Steel - Hot rolled bars for reinforced
https://echa.europa.eu/ concrete
FONDONORMA 316 NTP 339
FONDONORMA 316:2005 - Barras y rollos de acero NTP 339.186:2018 – Productos de acero. Barras de
con resaltes para uso como refuerzo estructural acero de baja aleación, soldables y corrugadas, para
refuerzo de concreto armado. Requisitos.
GaBi ts Software
GaBi ts: Software and databasis for life cycle NTP 341
engineering. LBP, University of Stuttgart und PE NTP 341.031:2018 – Productos de Acero. Barras de
International, 2013. acero al carbono, corrugadas, para refuerzo de
concreto armado. Requisitos.
GaBi ts Documentation
GaBi ts: Documentation of the GaBi datasets for life NTC 2289
cycle engineering. LBP, Universitity of Stuttgart and PE NTC 2289:2020 - Low-alloy steel deformed and plain
International, 2011. http://documentation.gabi- bars for concrete reinforcement
software.com.
PCR 2016, Part A
IBU 2016 Product Category Rules for Building-Related Products
Institut Bauen und Umwelt e.V.: General Instructions and Services, Calculation Rules for the Life Cycle
for the EPD programme of Institut Bauen und Umwelt Assessment and Requirements on the Project Report.
e.V. Version 2.0, Berlin: Institut Bauen und Umwelt Institut Bauen und Umwelt e.V. (IBU) March 2016
e.V., 2021. www.ibu-epd.com www.bau-umwelt.de
IRAM 500-207 PCR 2017, Part B
IRAM-IAS U 500-207:2017 - Hot rolled deformed Requirements on the EPD for Structural Steel - Institut
weldable steel bars for reinforcement of concrete Bauen und Umwelt e.V., Königswinter (pub.): From the
structures. range of Environmental Product Declarations of
Institute Construction and Environment e.V. (IBU),
IRAM 500-528 2017
IRAM-IAS U 500-528:2020 - Hot rolled deformed steel
bars for reinforcement of con-crete structures PNA 4-007-99
6 Environmental Product Declaration ArcelorMittal – Reinforcing steel in bars
NP 4-007:99 - Barras de acero conformadas, Life cycle assessment (LCA) methodology report
laminadas en caliente, para armaduras en estructuras http://www.worldsteel.org/publications/ABNT NBR
de hormigón. 6118:2014 - Design of concrete structures —
Procedure
Steel Recycling
Steel recycling rates at a glance, 2007 Steel recycling
rates; Steel Recycling Institute.
Worldsteel, 2017
7 Environmental Product Declaration ArcelorMittal – Reinforcing steel in bars
Publisher
Institut Bauen und Umwelt e.V. Tel +49 (0)30 3087748- 0
Panoramastr. 1 Fax +49 (0)30 3087748- 29
10178 Berlin Mail info@ibu-epd.com
Germany Web www.ibu-epd.com
Programme holder
Institut Bauen und Umwelt e.V. Tel +49 (0)30 - 3087748- 0
Panoramastr 1 Fax +49 (0)30 – 3087748 - 29
10178 Berlin Mail info@ibu-epd.com
Germany Web www.ibu-epd.com
Author of the Life Cycle
Assessment Tel 0800 015 1221
ArcelorMittal Brasil Fax -
Av. Carandaí, 1115 - Funcionários Mail
25 an arcelormittalnet@arcelormittal.co
30130 -915 - Belo Horizonte m.br
Brazil Web
http://www.arcelormittal.com.b
r/
Owner of the Declaration
ArcelorMittal Brasil Tel 0800 015 1221
Av. Carandaí, 1115 - Funcionários Fax -
25 an Mail
30130 -915 - Belo Horizonte arcelormittalnet@arcelormittal.co
Brazil m.br
Web
http://www.arcelormittal.com.b
r/
