ENVIRONMENTAL PRODUCT DECLARATION
as per ISO 14025 and EN 15804+A2
Owner of the Declaration Kvadrat Acoustics A/S
Publisher Institut Bauen und Umwelt e.V. (IBU)
Programme holder Institut Bauen und Umwelt e.V. (IBU)
Declaration number EPD-KVC-20240080-CBA1-EN
Issue date 10.06.2024
Valid to 09.06.2029
Kvadrat Acoustics Track
Kvadrat Acoustics
www.ibu-epd.com | https://epd-online.com
General Information
Kvadrat Acoustics Kvadrat Acoustics Track
Programme holder Owner of the declaration
IBU – Institut Bauen und Umwelt e.V. Kvadrat Acoustics A/S
Hegelplatz 1 Orient Plads 1, 1
10117 Berlin 2150 Nordhavn
Germany Denmark
Declaration number Declared product / declared unit
EPD-KVC-20240080-CBA1-EN 1m2 configurable acoustic frame system
This declaration is based on the product category rules: Scope:
Textile covered acoustic frame systems, 01.08.2021 The declaration covers the average product Kvadrat Acoustics Track with
(PCR checked and approved by the SVR) an ABS frame and the Trevira CS textile option CASA. The Kvadrat
Acoustics Track is a configurable textile-covered acoustic frame system
from the company Kvadrat Acoustics. It is available with an ABS frame in
Issue date customized sizes ranging from 1000 mm x 1000 mm x 25 mm to 6000 mm
x 3000 mm x 25 mm (L x W x H) and the textile option CASA under the
10.06.2024
textile series Trevira CS. The product is declared as a kit since it is
available by a single manufacturer as a set of multiple separate
components, which are assembled at the building site. All products
Valid to
included in this average EPD are produced in Kvadrat Acoustics site in
09.06.2029 United Kingdom and distributed to the market of the United Kingdom. The
products' components (including the Trevira CS textile CASA) are
manufactured by Kvadrat Acoustics suppliers located in United States of
America (Illinois) and Europe (Germany, Czech Republic, United
Kingdom). Production data were collected for the year 2022.
The owner of the declaration shall be liable for the underlying information
and evidence; the IBU shall not be liable with respect to manufacturer
information, life cycle assessment data and evidences.
The EPD was created according to the specifications of EN 15804+A2. In
the following, the standard will be simplified as EN 15804.
Dipl.-Ing. Hans Peters
Verification
(Chairman of Institut Bauen und Umwelt e.V.)
The standard EN 15804 serves as the core PCR
Independent verification of the declaration and data according to ISO
14025:2011
internally X externally
Florian Pronold Dr.-Ing. Nikolay Minkov,
(Managing Director Institut Bauen und Umwelt e.V.) (Independent verifier)
1 Environmental Product Declaration - Kvadrat Acoustics - Kvadrat Acoustics Track
Product
The constituents of the product are shown in the table below.
Product description/Product definition
Packaging materials are not included. The Kvadrat Acoustics
Kvadrat Acoustics Track with ABS profile and Trevira CS CASA Track system consists of an ABS frame, a layer of mineral glass
textile is a site-fabricated acoustical wall system, which wool absorber, Trevira CS CASA textile (polyester textile) for
stretches textile over semi-rigid acoustic padding to control the panel's wear. Installation staples (galvanised steel) are also
sound and add to the aesthetic design of interior spaces. The included in the product kit. The amount of staples is 0.17 kg/m2
product is available in customized sizes and different textile
of Kvadrat Acoustics Track. The sales packaging includes
options under the trade name Kvadrat Acoustics Track. This
corrugated cardboard (tubes for ABS frame), galvanised steel
EPD includes only the Kvadrat Acoustics Track with ABS frame
(end-caps for tubes), core board and high density polyethylene
and Trevira CS textile CASA. The product is declared as a
(HD PE) film packaging for the Trevira CS CASA textile roll.
construction product 'kit', since it consists of multiple separate
components and is placed on the market by a single
This product does not contain substances listed in the
manufacturer. The system consists of a single-sided layer of
candidate list (date: 25.06.2020) exceeding 0.1 percentage by
tensioned textile, attached to an ABS frame profile, over a
mass.
mineral-based acoustic core.
Name Value Unit
For the use and application of the product, the respective
national provisions at the place of use apply, in Germany for ABS frame (ABS profile) 13.02 wt-%
example the Building Codes of the federal states and the Sound absorber (mineral glass wool) 74.88 wt-%
corresponding national specifications. Trevira CS CASA textile (polyester textile) 6.09 wt-%
Staples for frame (galvanised steel) 4.93 wt-%
Application
Kvadrat Acoustics Track controls sound and adds to the Staples for absorbent (galvanised steel) 1.08 wt-%
aesthetic design of interior spaces. The system is intended for
interior walls and is particularly well suited for spaces with Manufacturing and assembly
severe to moderate need for sound absorption, large free wall The ABS frame profile is manufactured by a supplier in Illinois,
surfaces, and late changes as the tracks are built on-site. It is United States of America. The rest of the components are
installed directly on a wall substrate and can be applied in manufactured by Kvadrat Acoustics suppliers, located in
many different markets, architectural needs and acoustic Europe. The components are delivered to Kvadrat Acoustics
environments. site in the United Kingdom, where they are stored temporarily
and assembled into a kit before being transported to the
Technical Data
application sites. Kvadrat Acoustics Track is assembled and
The product has a sound adsorption class C according to ISO
installed at the building site (United Kingdom). This procedure
11654 with a sound absorption coefficient of 0.6 (ISO 354). The
includes cutting the frame profiles, absorber, and textile to the
fire performance is C-s2,d0. The dimensions of the system after
required size and installing the panel. Most of these activities
its installation in the building site are:
are done manually without any material consumption. An
electric staple gun compressor is used for the installation of
Typical size panel: 2700 mm x 1300 mm x 25 mm
staples. After the building or the product reaches its end-of-life
Min. size panel: 1000 mm x 1000 mm x 25 mm
stage, the system is removed and dismantled. This process
Max. size panel: 6000 mm x 3000 mm x 25 mm
requires mostly manual work.
The components comprising the product kit are delivered at the
building site with the following dimensions. The components
arrive at the building site in fixed dimensions however, the
number of component pieces differs across systems with
different sizes.
ABS frame (profiles): 2700 mm x 26 mm x 23 mm
Mineral glass wool absorber: 1200 mm x 1200 mm x 22 mm
Trevira CS CASA textile (roll): 400 mm x 400 mm x 1500 mm
Constructional data
Name Value Unit
Sound absorption class cf. ISO 11654 C -
Sound absorption coefficient cf. ISO-354 0.6 -
Dimensions max. (L x W x H) 6000x3000x25 mm
Dimensions min. (L x W x H) * 1000x1000x25 mm
Fire performance cf. EN-13501-1 C-s2,d0 -
* Smaller sizes are available from Kvadrat Acoustics, but are
not covered by the EPD.
Performance data of the product with respect to its
characteristics in accordance with the relevant technical Reference service life
provision (no CE-making). The Service Life declared by the manufacturer is 50 years.
Base materials/Ancillary materials
2 Environmental Product Declaration - Kvadrat Acoustics - Kvadrat Acoustics Track
LCA: Calculation rules
Declared Unit The construction process stage (A4-A5) includes:
The declared unit is 1 m2 configurable acoustic frame system A4 - Transport of the kit from Kvadrat Acoustics site to the
with weight of 2.79 kg/m2. The final LCA results refer to a building site.
typical Kvadrat Acoustics Track size of 2700 mm x 1300 mm x A5 - Installation of Kvadrat Acoustics Track system at the
25 mm (L x W x H), which represents all the product sizes application site including in-situ processing of components
included in this EPD. All Kvadrat Acoustics Track sizes, (cutting the components to the correct size, installing the
included in this EPD, consist of the same type of components staples). Module A5 also includes the transport and processing
and no variation takes place regarding the components' type. of waste (material loss, packaging) generated in the application
The amount of each component per declared unit differs site.
between different product sizes. No component was included
as an unweighted average. The results correspond to a typical The end-of-life stage includes:
Kvadrat Acoustics Track size of 1300 mm x 2700 mm x 25 mm C1 - Deconstruction and dismantling of the system. The manual
(L x W x H), which represents all the product sizes included in dismantling impact of the system is considered negligible and
this EPD. Finally, this EPD covers only the Trevira CS textile module C1 is reported without any impacts.
option CASA, which is a polyester textile. C2 - Transport of waste from the building site to Material
Recovery Facilities (MRF), as well as transport of recyclable
Declared unit
and non-recyclable waste from MRF to recycling facilities and
The declared unit is 1 m2 configurable acoustic frame system
landfill, respectively.
with a conversion factor of 2.79 kg/m2. C3 - Waste processing for dismantling the system into
Name Value Unit components and sorting the components/materials to waste for
Declared unit 1 m2 material recovery and landfill.
C4 - Disposal of non-recyclable components/materials (textile,
Grammage 2.79 kg/m2
absorber) to landfill.
Content of frame (based on weight) 13.02 % Module D includes reuse, recovery and/or recycling potentials.
Content of textile membrane (based on weight) 6.09 % Benefits originating from the recycling of material loss and
Content of in-fill (based on weight) 74.88 % metal components after reaching their end-of-life stage, as well
as the incineration of plastic packaging, were considered in
Deviation from frame (max. kg/m²)* 75.49 %
module D
Panel size typical 3.51 m2
Layer thickness 0.025 m
Geographic Representativeness
* The maximum percentage deviation of the frame refers to the
Land or region, in which the declared product system is
minimum size (1000 mm x 1000 mm x 25 mm). For the
manufactured, used or handled at the end of the product´s
maximum size (3000 mm x 6000 mm x 25 mm) the deviation
lifespan: Europe
is -56.13 %.
The LCA values included in this EPD are considered robust. Comparability
The reference product groups considered in this EPD are
Basically, a comparison or an evaluation of EPD data is only
assembled into kits in the same production/storing facility, while
possible if all the data sets to be compared were created
the components are manufactured by the same suppliers. In
according to EN 15804 and the building context, respectively
addition, the background datasets used are representative of
the product-specific characteristics of performance, are taken
the geographical scope, technologies and production
into account.
processes used. Therefore, variations in geography are not
relevant. Plant production data for the period of 2022-2023
Data Quality
were collected.
Background data were retrieved from Managed LCA Content
database (formerly known as GaBi database) version 2022.2
System boundary
provided by Sphera and Ecoinvent database. The quality of
The EPD is of the type cradle-to-gate with options, modules A4,
foreground and background data is considered very good and
A5, C1-C4 and D. The product stage (A1-A3) includes:
all major processes are represented with data of good quality in
A1 - Raw material extraction, processing, processing of
compliance with the stated criteria from the PCR. In addition,
secondary material input (e.g. recycling processes) and
the conservative approach was adopted when foreground data
production of the components. The production of excess
quality was insufficient. The background data are up to date
components to compensate for material losses during the
and the temporal data quality requirements of the PCR are
installation phase, as well as the production of ancillary
generally met. The temporal span of the background data used
materials (installation screws), are accounted for in module A1
ranges from 2015 to 2025 and no data are more than 10 years
because the product is declared as a kit.
old. Allocation of energy used for storing, moving and
A2 - Transport of components and packaging from the suppliers
assembling the product kit in module A3 was performed. The
to Kvadrat Acoustics site.
allocation key is the area occupied by the Kvadrat Acoustics
A3 - Assembly of components into a product kit. The production
Track in the warehouse since the activities are dependent on
of sales packaging (plastic, core board, corrugated cardboard
the product's area.
tubes, steel end-caps packaging for the textile and frame) is
included in module A3.
LCA: Scenarios and additional technical information
Characteristic product properties of biogenic carbon
3 Environmental Product Declaration - Kvadrat Acoustics - Kvadrat Acoustics Track
The Kvadrat Acoustics Track with the Trevira CS textile CASA
do not include any materials with biogenic carbon content. The
Reference service life
product's packaging includes biogenic carbon due to the
Name Value Unit
presence of a core board and corrugated cardboard in the
Trevira CS textile CASA and ABS frame packaging. (Technical) Service life 50 years
Information on describing the biogenic Carbon Content at End of life (C1 - C4)
factory gate
Name Value Unit
Note: 1 kg of biogenic carbon is equivalent to 44/12 kg of CO .
2 % incineration with
ABS frame 100
Name ValueUnit energy recovery
kg Galvanised steel staples EoL
Biogenic carbon content in product - 100 % recycling
C scenario
Biogenic carbon content in accompanying kg Mineral glass wool absorber
0.057 100 % landfill
packaging (core board) C EoL scenario
Trevira CS textile EoL
100 % landfill
Technical scenario information for the declared modules A4, A5, scenario
C1-C4 and D is provided in the following tables. The electricity Collected separately waste
- kg
consumption and material loss in module A5 were measured for type
the typical Kvadrat Acoustics Track size based on the actual Collected as mixed
activities taking place during the system's installation at the construction waste 2.79 kg
building site. An end-of-life (EoL) scenario was established for
Recycling 0.17 kg
the packaging waste in module A5 which assumes that the core
Energy recovery 0.36 kg
board and plastic packaging waste is recycled, based on
Kvadrat Acoustics activities. Landfilling 2.26 kg
Transport to the building site (A4) Reuse, recovery and/or recycling potentials (D), relevant
Name Value Unit scenario information
Litres of fuel 0.0221 l/100km Name Value Unit
Transport distance 154 km Replaced primary galvanized steel (staples) 0.16 kg
Capacity utilisation (including empty runs) 51 % 8.38E-
Replaced primary ABS (material loss, frame) kg
Gross density of products transported 124.52 kg/m3 03
Replaced primary polyester textile (material loss, 2.04E-
kg
Installation into the building (A5) Trevira textile CASA 02
Name Value Unit Replaced primary galvanised steel (sales 8.32E-
kg
Electricity consumption 0.0128 kWh packaging, ABS frame) 03
Material loss (ABS frame, Trevira CS textile Replaced primary HD PE (sales packaging, 3.18E-
0.0295 kg kg
CASA) Trevira CS textile CASA) 03
3.53E- Replaced electricity (grid mix) 0.61 kWh
Plastic packaging for recycling kg
03 Replaced thermal energy (natural gas) 4.02 MJ
1.40E-
Core board packaging for recycling kg
01
8.76E-
Galvanised steel packaging for recycling kg
03
4 Environmental Product Declaration - Kvadrat Acoustics - Kvadrat Acoustics Track
LCA: Results
DESCRIPTION OF THE SYSTEM BOUNDARY (X = INCLUDED IN LCA; MND = MODULE OR INDICATOR NOT DECLARED; MNR
= MODULE NOT RELEVANT)
Benefits and
Construction loads beyond
Product stage Use stage End of life stage
process stage the system
boundaries
la ire ta m w a Ry lp p u s tro p s n a rT g n iru tc a fu n a M e h t m o rf tro p s n a rTe tis e h t o t e ta g y lb m e s s A e s U e c n a n e tn ia M ria p e R tn e m e c a lp e R tn e m h s ib ru fe R y g re n e la n o ita re p Oe s u re ta w la n o ita re p Oe s u n o itc u rts n o c -e Dn o itilo m e d tro p s n a rT g n is s e c o rp e ts a W la s o p s iD -e s u e R-y re v o c e R-g n ilc y c e Rla itn e to p
A1 A2 A3 A4 A5 B1 B2 B3 B4 B5 B6 B7 C1 C2 C3 C4 D
X X X X X MND MND MNR MNR MNR MND MND X X X X X
RESULTS OF THE LCA - ENVIRONMENTAL IMPACT according to EN 15804+A2: 1 m² Kvadrat Acoustics Track
Parameter Unit A1 A2 A3 A4 A5 C1 C2 C3 C4 D
GWP-total kg CO 2 eq 6.32E+00 2.73E-01 9.47E-03 1.02E-01 2.5E-01 0 1.09E-01 7.75E-01 2.51E-01 -7.79E-01
GWP-fossil kg CO 2 eq 6.57E+00 2.71E-01 2.6E-01 1.01E-01 3.86E-02 0 1.08E-01 7.75E-01 5.28E-02 -7.76E-01
GWP-
biogenic kg CO 2 eq -2.51E-01 -5.55E-04 -2.51E-01 -2.8E-04 2.12E-01 0 -2.96E-04 -2.69E-05 1.99E-01 -2.85E-03
GWP-luluc kg CO 2 eq 7.73E-03 2.11E-03 5.86E-04 9.51E-04 1.89E-04 0 1.01E-03 5.95E-05 1.07E-04 -2.88E-04
ODP kg CFC11 eq 7.53E-09 3.4E-14 1.07E-09 1.34E-14 1.38E-09 0 1.42E-14 9.74E-14 9.95E-14 -3.44E-12
AP mol H+ eq 2.96E-02 1.1E-03 1.24E-03 1.48E-04 9.34E-05 0 1.79E-04 6.39E-04 2.83E-04 -1.26E-03
EP-
kg P eq 2.99E-05 8.54E-07 2.53E-05 3.75E-07 1.33E-06 0 3.98E-07 5.18E-08 2.37E-06 -3.96E-07
freshwater
EP-marine kg N eq 5.51E-03 4.47E-04 2.92E-04 5.31E-05 3.52E-05 0 6.81E-05 3.15E-04 1.78E-04 -3.51E-04
EP-terrestrial mol N eq 1.19E-01 5.01E-03 2.78E-03 6.33E-04 3.67E-04 0 7.98E-04 3.56E-03 8.55E-04 -3.79E-03
kg NMVOC
POCP 1.4E-02 1.2E-03 6.99E-04 1.29E-04 1.01E-04 0 1.6E-04 8.09E-04 3.05E-04 -1.1E-03
eq
ADPE kg Sb eq 1.18E-05 1.74E-08 6.84E-07 6.81E-09 6E-08 0 7.21E-09 8.68E-09 1.76E-09 -4.57E-08
ADPF MJ 1.28E+02 3.65E+00 4E+00 1.4E+00 5.61E-01 0 1.48E+00 4.01E-01 5.92E-01 -1.15E+01
m3 world eq
WDP 9.72E-01 3.08E-03 7.46E-02 1.24E-03 2.16E-03 0 1.31E-03 9.99E-02 4.31E-03 -1.67E-02
deprived
GWP = Global warming potential; ODP = Depletion potential of the stratospheric ozone layer; AP = Acidification potential of land and water; EP =
Eutrophication potential; POCP = Formation potential of tropospheric ozone photochemical oxidants; ADPE = Abiotic depletion potential for non-fossil
resources; ADPF = Abiotic depletion potential for fossil resources; WDP = Water (user) deprivation potential)
RESULTS OF THE LCA - INDICATORS TO DESCRIBE RESOURCE USE according to EN 15804+A2: 1 m² Kvadrat Acoustics
Track
Parameter Unit A1 A2 A3 A4 A5 C1 C2 C3 C4 D
PERE MJ 1.79E+01 2.31E-01 1.97E+00 1.02E-01 6.76E-02 0 1.08E-01 6.38E-02 8.39E-02 -2.77E+00
PERM MJ 3.01E+00 0 1.7E+00 0 0 0 0 0 0 0
PERT MJ 2.1E+01 2.31E-01 3.67E+00 1.02E-01 6.76E-02 0 1.08E-01 6.38E-02 8.39E-02 -2.77E+00
PENRE MJ 1.1E+02 3.7E+00 3.87E+00 1.4E+00 5.62E-01 0 1.49E+00 1.46E+01 5.93E-01 -1.15E+01
PENRM MJ 1.9E+01 0 1.54E-01 0 0 0 0 -1.42E+01 0 0
PENRT MJ 1.29E+02 3.7E+00 4.02E+00 1.4E+00 5.62E-01 0 1.49E+00 4.01E-01 5.93E-01 -1.15E+01
SM kg 1.25E+00 0 7.16E-02 0 0 0 0 0 0 0
RSF MJ 0 0 0 0 0 0 0 0 0 0
NRSF MJ 0 0 0 0 0 0 0 0 0 0
FW m3 3.09E-02 2.59E-04 2.07E-03 1.11E-04 9.79E-05 0 1.18E-04 2.35E-03 1.31E-04 -1.6E-03
PERE = Use of renewable primary energy excluding renewable primary energy resources used as raw materials; PERM = Use of renewable primary
energy resources used as raw materials; PERT = Total use of renewable primary energy resources; PENRE = Use of non-renewable primary energy
excluding non-renewable primary energy resources used as raw materials; PENRM = Use of non-renewable primary energy resources used as raw
materials; PENRT = Total use of non-renewable primary energy resources; SM = Use of secondary material; RSF = Use of renewable secondary fuels;
NRSF = Use of non-renewable secondary fuels; FW = Use of net fresh water
RESULTS OF THE LCA – WASTE CATEGORIES AND OUTPUT FLOWS according to EN 15804+A2:
1 m² Kvadrat Acoustics Track
Parameter Unit A1 A2 A3 A4 A5 C1 C2 C3 C4 D
HWD kg 8.31E-06 1.12E-11 1.03E-08 4.35E-12 5.89E-12 0 4.61E-12 2.22E-11 2.38E-11 -1.83E-07
NHWD kg 2.43E-01 5.06E-04 2.57E-02 2.14E-04 1.66E-03 0 2.27E-04 2.41E-02 2.22E+00 -1.69E-03
RWD kg 3.61E-03 7.28E-06 1.77E-04 2.63E-06 2.3E-05 0 2.78E-06 1.17E-05 6.84E-06 -4.87E-04
CRU kg 0 0 0 0 0 0 0 0 0 0
MFR kg 0 0 1.93E-01 0 1.82E-01 0 0 1.68E-01 0 0
MER kg 0 0 0 0 0 0 0 3.63E-01 0 0
5 Environmental Product Declaration - Kvadrat Acoustics - Kvadrat Acoustics Track
EEE MJ 0 0 0 0 0 0 0 2.21E+00 0 0
EET MJ 0 0 0 0 0 0 0 4.02E+00 0 0
HWD = Hazardous waste disposed; NHWD = Non-hazardous waste disposed; RWD = Radioactive waste disposed; CRU = Components for re-use;
MFR = Materials for recycling; MER = Materials for energy recovery; EEE = Exported electrical energy; EET = Exported thermal energy
RESULTS OF THE LCA – additional impact categories according to EN 15804+A2-optional:
1 m² Kvadrat Acoustics Track
Parameter Unit A1 A2 A3 A4 A5 C1 C2 C3 C4 D
Disease
PM 3.17E-07 2.25E-08 1.41E-08 1.29E-09 1.23E-09 0 1.22E-09 2.92E-09 3.32E-09 -1.59E-08
incidence
IR kBq U235 eq 5.38E-01 9.93E-04 1.69E-02 3.92E-04 3.39E-03 0 4.15E-04 1.8E-03 8.57E-04 -4.99E-02
ETP-fw CTUe 1.71E+02 2.67E+00 2.03E+00 1E+00 2.59E-01 0 1.06E+00 2.06E-01 6.32E-01 -2.64E+00
HTP-c CTUh 5.23E-09 5.21E-11 2.95E-10 2.03E-11 1.4E-11 0 2.15E-11 8.13E-12 4.35E-11 -6.35E-10
HTP-nc CTUh 1.34E-07 2.15E-09 1.67E-09 9.04E-10 2.93E-10 0 9.58E-10 5.93E-10 4.59E-09 -2.21E-09
SQP SQP 6.94E+01 1.3E+00 7.24E+00 5.84E-01 1.94E-01 0 6.19E-01 9.44E-02 1.17E-01 -1.83E+00
PM = Potential incidence of disease due to PM emissions; IR = Potential Human exposure efficiency relative to U235; ETP-fw = Potential comparative
Toxic Unit for ecosystems; HTP-c = Potential comparative Toxic Unit for humans (cancerogenic); HTP-nc = Potential comparative Toxic Unit for humans
(not cancerogenic); SQP = Potential soil quality index
Disclaimer for the indicator 'potential Human exposure efficiency relative to U235': This impact category deals mainly with the eventual
impact of low-dose ionizing radiation on human health of the nuclear fuel cycle. It does not consider effects due to possible nuclear
accidents, occupational exposure or radioactive waste disposal in underground facilities. Potential ionizing radiation from the soil,
radon and from some construction materials is also not measured by this indicator.
Disclaimer for the indicators 'abiotic depletion potential for fossil resources', 'abiotic depletion potential for non-fossil resources', 'water
(user) deprivation potential, deprivation-weighted water consumption', 'potential comparative toxic unit for ecosystems', 'potential
comparative toxic unit for humans - cancer effects', 'potential comparative toxic unit for humans – non-cancer effects', 'potential soil
quality index': The results of this environmental impact indicator shall be used with care as the uncertainties on these results are high
or as there is limited experience with the indicator.
The major contributor across all environmental impact indicators (except GWP-biogenic) is module A1. This is expected since the
Kvadrat Acoustics Track is a product kit, the entire manufacturing of components takes place in Kvadrat Acoustics A/S upstream supply
chain. Modules A3 and A1 have the lowest negative impact in the GWP-biogenic indicator due to the production of core
board/corrugated cardboard (sales packaging) and wooden pallets (incoming packaging), respectively. In addition, the activities taking
place in Kvadrat Acoustics sites relate to the storing, moving and preparing of the product kit which does not require high energy
consumption. Therefore, module A3 has a low contribution to the environmental impacts. Materials with secondary content are used in
the mineral glass wool and are included in some secondary datasets. Finally, the use of secondary fuels is included in secondary
datasets yet no secondary fuels are used in Kvadrat Acoustics sites.
References
ISO 11654
ISO 11654, 1997: Acoustics — Sound absorbers for use in GaBi LCA software and database
buildings — Rating of sound absorption The LCA modelling software is GaBi program version
10.5.1.125 with corresponding databases from Sphera
EN 13501-1 Solutions GmbH. Documentation
EN13501-1, 2018: Fire classification of construction products www.gabisoftware.com/support/gabi.
and building elements - Part 1: Classification using data from
reaction to fire tests. IBU PCR 2023, Part B
Requirements on the EPD for Textile covered acoustic frame
ISO 14025 systems. Version 2.0; 2023.
DIN EN ISO 14025:2011-10, Environmental labels and
declarations — Type III environmental declarations — IBU PCR 2019, Part A
Principles and procedures. The Product Category Rules for Building-Related Products and
Services, Part A: Calculation Rules for the Life Cycle
EN 15804 Assessment and Requirements on the Project Report according
EN 15804:2019+A2 (in press), Sustainability of construction to EN 15804+A2:2019, Version 1.4. from Institut Bauen und
works — Environmental Product Declarations — Core rules for Umwelt e.V. (IBU)
the product category of construction products.
IBU 2021
ISO 354 Institut Bauen und Umwelt e.V.: General Instructions for the
ISO 354, 2013: Acoustics - Measurement of sound absorption EPD programme of Institut Bauen und Umwelt e.V. Version 2.0,
in a reverberation room. Berlin: Institut Bauen und Umwelt e.V., 2021. www.ibu-
epd.com.
ECHA Candidate List
List of substances of very high concern considered for approval
(status 25.06.2020) according to Article 59
para. 10 of the REACH Regulation. European Chemicals
Agency
6 Environmental Product Declaration - Kvadrat Acoustics - Kvadrat Acoustics Track
Publisher
Institut Bauen und Umwelt e.V. +49 (0)30 3087748- 0
Hegelplatz 1 info@ibu-epd.com
10117 Berlin www.ibu-epd.com
Germany
Programme holder
Institut Bauen und Umwelt e.V. +49 (0)30 3087748- 0
Hegelplatz 1 info@ibu-epd.com
10117 Berlin www.ibu-epd.com
Germany
Author of the Life Cycle Assessment
FORCE Technology +4543250856
Park Alle 345 chme@forcetechnology.com
2605 Brøndby www.forcetechnology.com
Denmark
Owner of the Declaration
Kvadrat Acoustics A/S +4589531866
Orient Plads 1, 1 kvadratacoustics@kvadrat.org
2150 Nordhavn www.kvadratacoustics.com
Denmark
7 Environmental Product Declaration - Kvadrat Acoustics - Kvadrat Acoustics Track
