ENVIRONMENTAL PRODUCT DECLARATION
as per ISO 14025 and EN 15804+A2
Owner of the Declaration Saarstahl Rail
Publisher Institut Bauen und Umwelt e.V. (IBU)
Programme holder Institut Bauen und Umwelt e.V. (IBU)
Declaration number EPD-SAA-20230151-CBD1-EN
Issue date 14.07.2023
Valid to 13.07.2028
Pure Steel+ Rail
Saarstahl Rail
www.ibu-epd.com | https://epd-online.com
General Information
Saarstahl Rail Pure Steel+ Rail
Programme holder Owner of the declaration
IBU – Institut Bauen und Umwelt e.V. Saarstahl Rail
Hegelplatz 1 Rue du Maréchal Foch 164
10117 Berlin 57705 Hayange Cedex
Germany France
Declaration number Declared product / declared unit
EPD-SAA-20230151-CBD1-EN Rail product / 1 metric tonne
This declaration is based on the product category rules: Scope:
Rails forming a track for vehicles, 01.08.2021 The EPD declaration applies to 1 metric tonne of rail product manufactured
(PCR checked and approved by the SVR) at Saarstahl Rail.
The "Pure Steel+" rails from Saarstahl Rail are high-quality rail products
Issue date from the Saarstahl Rail hot rolling mill in Hayange (France) with EAF
based pre-material from Saarstahl Ascoval in St. Valenciennes (France).
14.07.2023
Both subsidaries Saarstahl Rail and Saarstahl Ascoval do belong to the
Saarstahl group, specialist in steel long products, based in Völklingen
(Germany).
Valid to
13.07.2028 The LCA does represent 100% EAF pre-material based rails within the
reference year of 2021.
The owner of the declaration shall be liable for the underlying information
and evidence; the IBU shall not be liable with respect to manufacturer
information, life cycle assessment data and evidences.
The EPD was created according to the specifications of EN 15804+A2. In
the following, the standard will be simplified as EN 15804.
Verification
The standard EN 15804 serves as the core PCR
Dipl.-Ing. Hans Peters
Independent verification of the declaration and data according to ISO
(Chairman of Institut Bauen und Umwelt e.V.)
14025:2011
internally X externally
Florian Pronold Prof. Dr. Birgit Grahl,
(Managing Director Institut Bauen und Umwelt e.V.) (Independent verifier)
1 Environmental Product Declaration - Saarstahl Rail - Pure Steel+ Rail
Product
crossings. The steel grades are designed and adapted to the
Product description/Product definition applications.
The products of Saarstahl Rail refer to rails (Vignole rail, tong
rail, grooved rail, check rail and piste), that are manufactured Technical Data
and delivered as approximately 100 different profiles and 25 The EPD refers to all EAF based products from Saarstahl Rail
grades from 6 m to 108 m. They are compliant to applicable in a variety of different steel grades, dimensions, shapes and
European and international standards, guidelines and as-delivered conditions.
specifications depending on the use and application of the
Constructional data
product. The respective national provisions at the place of use
Name Value Unit
apply. The products com from blooms which are reheated and
rolled at high temperatures going through a series of stands of Density 7850 kg/m3
rotating cylinders. Steel alloy composition and process Modulus of elasticity 2.07/10^5 N/mm2
parameters are set to guarantee the required grade and profile.
Tensile strength >680 N/mm2
Some rails for special applications (heat treated rails) are
Grade of material R200 R220 R260 R260Mn
reheated in an induction furnace line and cooled with
according to the R260Cr R320Cr R350HT -
pressurized air to increase the hardness of the steel. For the
delivery standards R350LHT R370CrHT R400HT
placing on the market in the European Union/European Free
Trade Association (EU/EFTA) (with the exception of Grade of material according to the delivery standards:
Switzerland) the following legal provisions apply: EN13674-1; EN13674-2; EN13674-3; EN13674-4; EN14811.
Directive (EU) 2016/797 of the European Parliament and of the Performance data of the product in accordance with the
Council of 11 May 2016 on the interoperability of the rail system declaration of performance with respect to its essential
within the European Union, Commission regulation 1299/2014 characteristics.
of 18th November 2014 concerning a technical specification for
interoperability relating to the infrastructure subsystem of the Base materials/Ancillary materials
rail system in the European Union, and to the Commission The "Pure Steel+" products of Saarstahl Rail are manufactured
Implementing Regulations (EU) 2019/776 and (EU) 2020/387. with 100% continuously cast bloom (with about 97% scrap and
alloying elements) pre-material produced from EAF at Saarstahl
and the harmonised standards based on these provisions: Ascoval. The overall composition of the steel grades does
depend on the customer specification and application use of
EN 13674-1:2011+A1:2017, Railway applications – Track – Rail the final product.
– Part 1: Vignole railway rails 46 kg/m and above
EN 13674-2:2019, Railway applications – Track – Rail – Part 2: The product contains substances in the European Chemicals
Switch and crossing rails used in conjunction with Vignole Agency (ECHA) candidate list/ (15 January 2019) above 0.1
railway rails 46 kg/m and above mass %: no.
EN 13674-3:2006+A1:2010, Railway applications – Track – Rail
– Part 3: Check rails The product contains further carcinogenic, mutagenic,
EN 13674-4:2020, Railway applications - Track - Rail - Part 4: reprotoxic (CMR) substances of category 1A or 1B that are not
Vignole railway rails from 27 kg/m to, but excluding 46 kg/m in the candidate list, above 0.1 mass % in at least one sub-
EN 14811:2019, Railway applications – Track – Special product: no.
purpose rail – Grooved and associated construction
Biocides have been added to the construction product, or the
The CE-marking takes into account the proof of conformity with product has been treated with biocides (a treated product
the respective harmonized standards based on the legal pursuant to the Biocidal Product Regulation (EU) No.
provisions above. 528/2012): no.
For the application and use the respective national provisions
Reference service life
apply.
The specification of a reference service life of any rail product is
Application based on the multiple purposes and application options (e.g.
Saarstahl rail is specialized in the production of Vignole rail, regarding stress levels (high-speed traffic, mixed traffic, heavy
tong rail, grooved rail, check rail and piste for rubber tire metro loads, passenger traffic, urban traffic, switch technologies)).
at its location of Hayange. Typical applications for the rails The various rail options avalable, including the optimal choice
manufactured in Hayange are the high-speed lines, national of rail product or specification, do increase the lifetime
train networks for freight and passenger traffic, urban networks drastically. The service life of any rail product can be enhanced
as metro or tramway, heavy haul lines as mining or industrial by regular maintenance of the user.
networks and rail for the manufacturing of switches and
LCA: Calculation rules
Name Value Unit
Declared Unit
Declared unit 1 t
This environmental product declaration refers to a declared unit
of 1 ton of rail.
Density 7850 kg/m3
Conversion factor to 1 kg 0,001 -
Declared unit
This EPD covers Saarstahl rails of different profiles and grades
considered representative for all Saarstahl rail products. All rails
are in the same order of magnitude regarding the grade and
2 Environmental Product Declaration - Saarstahl Rail - Pure Steel+ Rail
there are no differences in environmental impact regarding the dismantling there is no processing for recycling in C3. There is
different shapes. no disposal (C4) as the considered End-of-Life scenario is
100% recycling.
System boundary
The life cycle assessment of Saarstahl Rail refers to a cradle- Module D (Benefits and loads beyond the system
to-gate analysis with options. The following life cycle phases boundary)
are taken into account: Module D describes the net benefits and loads for substituting
primary steel through steel recycling.
Module A1-A3 (Production Stage)
Module A1-A3 covers the upstream burdens of purchased Geographic Representativeness
materials (ferro-alloys, lime, dolomite, etc.) and energies Land or region, in which the declared product system is
(electricity, natural gas, etc.), their transports and the manufactured, used or handled at the end of the product´s
manufacturing at the production sites Ascoval and Hayange of lifespan: Global
Saarstahl Rail.
No packaging is needed for the delivery of the product.
Comparability
Module C1-C4 (End-of-Life Stage) Basically, a comparison or an evaluation of EPD data is only
At End-of-Life the steel material leaves the product system in possible if all the data sets to be compared were created
C3 for recycling in the next product system. For the dismantling according to EN 15804 and the building context, respectively
of the considered product (C1) and the transportation of the the product-specific characteristics of performance, are taken
dismantled components to their final EoL destination (C2) the into account. The background database from /GaBi database/
data are not robust enough to be considered. As the steel scrap was used to calculate the LCA.
produced End-of-Life reaches the end-of-waste state after
LCA: Scenarios and additional technical information
Characteristic product properties of biogenic carbon According to EN 15804+A2 it is requested to declare 100%
There is no biogenic carbon within the steel product. And there End-of-Life scenarios (here considered: 100% recycling).
is no packaging needed for the product under study.
End of life (C1 - C4)
Information on describing the biogenic carbon content at
Name Value Unit
factory gate
Collected separately waste type 1000 kg
Name ValueUnit
Recycling 1000 kg
kg
Biogenic carbon content in product -
C Reuse, recovery and/or recycling potentials (D), relevant
Biogenic carbon content in accompanying kg scenario information
-
packaging C Name Value Unit
Net flow of steel scrap -50,41 kg
3 Environmental Product Declaration - Saarstahl Rail - Pure Steel+ Rail
LCA: Results
The following table describes the LCA results for a declared unit of 1 ton of average Saarstahl rails.
DESCRIPTION OF THE SYSTEM BOUNDARY (X = INCLUDED IN LCA; ND = MODULE OR INDICATOR NOT DECLARED; MNR =
MODULE NOT RELEVANT)
Benefits and
Construction loads beyond
Product stage Use stage End-of-life stage
process stage the system
boundaries
la ire ta m w a Ry lp p u s tro p s n a rT g n iru tc a fu n a M e h t m o rf tro p s n a rTe tis e h t o t e ta g y lb m e s s A e s U e c n a n e tn ia M ria p e R tn e m e c a lp e R tn e m h s ib ru fe R y g re n e la n o ita re p Oe s u re ta w la n o ita re p Oe s u n o itc u rts n o c -e Dn o itilo m e d tro p s n a rT g n is s e c o rp e ts a W la s o p s iD -e s u e R-y re v o c e R-g n ilc y c e Rla itn e to p
A1 A2 A3 A4 A5 B1 B2 B3 B4 B5 B6 B7 C1 C2 C3 C4 D
X X X MND MND MND MND MNR MNR MNR MND MND X X X X X
RESULTS OF THE LCA - ENVIRONMENTAL IMPACT according to EN 15804+A2: 1 ton rail
Parameter Unit A1-A3 C1 C2 C3 C4 D
Global Warming Potential total (GWP-total) kg CO 2 eq 7.89E+02 ND ND 0 0 8.73E+01
Global Warming Potential fossil fuels (GWP-fossil) kg CO 2 eq 7.87E+02 ND ND 0 0 8.73E+01
Global Warming Potential biogenic (GWP-biogenic) kg CO 2 eq 1.25E+00 ND ND 0 0 -4.46E-02
Global Warming Potential luluc (GWP-luluc) kg CO 2 eq 1.8E-01 ND ND 0 0 1.8E-03
Depletion potential of the stratospheric ozone layer (ODP) kg CFC11 eq 3.39E-09 ND ND 0 0 1.91E-13
Acidification potential of land and water (AP) mol H+ eq 3.14E+00 ND ND 0 0 1.88E-01
Eutrophication potential aquatic freshwater (EP-freshwater) kg P eq 6.7E-04 ND ND 0 0 1.58E-05
Eutrophication potential aquatic marine (EP-marine) kg N eq 5.3E-01 ND ND 0 0 3.3E-02
Eutrophication potential terrestrial (EP-terrestrial) mol N eq 5.64E+00 ND ND 0 0 2.9E-01
Formation potential of tropospheric ozone photochemical oxidants kg NMVOC
1.52E+00 ND ND 0 0 1.34E-01
(POCP) eq
Abiotic depletion potential for non fossil resources (ADPE) kg Sb eq 8.63E-03 ND ND 0 0 2.18E-04
Abiotic depletion potential for fossil resources (ADPF) MJ 1.57E+04 ND ND 0 0 8.02E+02
m3 world eq
Water use (WDP) 1.89E+02 ND ND 0 0 1.62E+01
deprived
RESULTS OF THE LCA - INDICATORS TO DESCRIBE RESOURCE USE according to EN 15804+A2: 1 ton rail
Parameter Unit A1-A3 C1 C2 C3 C4 D
Renewable primary energy as energy carrier (PERE) MJ 2.58E+03 ND ND 0 0 -5.05E+01
Renewable primary energy resources as material utilization
MJ 0 ND ND 0 0 0
(PERM)
Total use of renewable primary energy resources (PERT) MJ 2.58E+03 ND ND 0 0 -5.05E+01
Non renewable primary energy as energy carrier (PENRE) MJ 1.57E+04 ND ND 0 0 8.02E+02
Non renewable primary energy as material utilization (PENRM) MJ 0 ND ND 0 0 0
Total use of non renewable primary energy resources (PENRT) MJ 1.57E+04 ND ND 0 0 8.02E+02
Use of secondary material (SM) kg 1.05E+03 ND ND 0 0 -5.04E+01
Use of renewable secondary fuels (RSF) MJ 0 ND ND 0 0 0
Use of non renewable secondary fuels (NRSF) MJ 0 ND ND 0 0 0
Use of net fresh water (FW) m3 7.91E+00 ND ND 0 0 3.66E-01
RESULTS OF THE LCA – WASTE CATEGORIES AND OUTPUT FLOWS according to EN 15804+A2:
1 ton rail
Parameter Unit A1-A3 C1 C2 C3 C4 D
Hazardous waste disposed (HWD) kg 9.86E-07 ND ND 0 0 6.19E-09
Non hazardous waste disposed (NHWD) kg 2.74E+01 ND ND 0 0 -1.22E+01
Radioactive waste disposed (RWD) kg 2.96E+00 ND ND 0 0 -9.97E-05
Components for re-use (CRU) kg 0 ND ND 0 0 0
Materials for recycling (MFR) kg 0 ND ND 1E+03 0 0
Materials for energy recovery (MER) kg 0 ND ND 0 0 0
Exported electrical energy (EEE) MJ 0 ND ND 0 0 0
Exported thermal energy (EET) MJ 0 ND ND 0 0 0
RESULTS OF THE LCA – additional impact categories according to EN 15804+A2-optional:
1 ton rail
Parameter Unit A1-A3 C1 C2 C3 C4 D
Disease
Incidence of disease due to PM emissions (PM) ND ND ND ND ND ND
incidence
Human exposure efficiency relative to U235 (IR) kBq U235 eq ND ND ND ND ND ND
Comparative toxic unit for ecosystems (ETP-fw) CTUe ND ND ND ND ND ND
Comparative toxic unit for humans (carcinogenic) (HTP-c) CTUh ND ND ND ND ND ND
4 Environmental Product Declaration - Saarstahl Rail - Pure Steel+ Rail
Comparative toxic unit for humans (noncarcinogenic) (HTP-nc) CTUh ND ND ND ND ND ND
Soil quality index (SQP) SQP ND ND ND ND ND ND
Disclaimer 1 – for the indicator “Potential Human exposure efficiency relative to U235”. This impact category deals mainly with the
eventual impact of low-dose ionizing radiation on human health of the nuclear fuel cycle. It does not consider effects due to possible
nuclear accidents, occupational exposure or radioactive waste disposal in underground facilities. Potential ionizing radiation from the
soil, radon and from some construction materials is also not measured by this indicator.
Disclaimer 2 – for the indicators “abiotic depletion potential for non-fossil resources”, “abiotic depletion potential for fossil resources”,
“water (user) deprivation potential, deprivation-weighted water consumption”, “potential comparative toxic unit for ecosystems”,
“potential comparative toxic unit for humans – cancerogenic”, “Potential comparative toxic unit for humans - not cancerogenic”,
“potential soil quality index”. The results of this environmental impact indicator shall be used with care as the uncertainties on these
results are high as there is limited experience with the indicator.
References
Standards
IBU Part A
EN 13674-1:2011+A1:2017 PCR - Part A: Calculation Rules for the Life Cycle Assessment
Railway applications – Track – Rail – Part 1: Vignole railway and Requirements on the Project Report according to EN
rails 46 kg/m and above 15804+A2:2019, version 1.3, Institut Bauen und Umwelt e.V.,
www.bau-umwelt.com, 2022
EN 13674-2:2020
Railway applications – Track – Rail – Part 2: Switch and IBU Part B
crossing rails used in conjunction with Vignole railway rails 46 PCR - Part B: Rails forming a track for vehicles, 01/08/2021
kg/m and above (PCR checked and approved by the SVR), Institut Bauen und
Umwelt e.V., www.bau-umwelt.com
EN 13674-3:2006+A1:2010
Railway applications – Track – Rail – Part 3: Check rails DIRECTIVE (EU) 2016/797 OF THE EUROPEAN
PARLIAMENT AND OF THE COUNCIL of 11 May 2016 on the
EN 13674-4:2020 interoperability of the rail system within the European Union
Railway applications - Track - Rail - Part 4: Vignole railway rails (recast)
from 27 kg/m to, but excluding 46 kg/m
COMMISSION REGULATION (EU) No 1299/2014 of 18
ISO 14025 November 2014 on the technical specifications for
EN ISO 14025:2011, Environmental labels and declarations — interoperability relating to the 'infrastructure' subsystem of the
Type III environmental declarations — Principles and rail system in the European Union
procedures.
Commission regulation 1299/2014 of 18th November 2014
EN 14811:2019 concerning a technical specification for interoperability relating
Railway applications – Track – Special purpose rail – Grooved to the infrastructure subsystem of the rail system in the
and associated construction European Union,
EN 15804 COMMISSION IMPLEMENTING REGULATION (EU) 2019/776
EN 15804:2012+A1 2013, Sustainability of construction works of 16 May 2019 amending Commission Regulations (EU) No
— Environmental Product Declarations — Core rules for the 321/2013, (EU) No 1299/2014, (EU) No 1301/2014, (EU) No
product category of construction products. 1302/2014, (EU) No 1303/2014 and (EU) 2016/919 and
Commission Implementing Decision 2011/665/EU as regards
EN 15804 the alignment with Directive (EU) 2016/797 of the European
EN 15804:2012+A2:2019+AC:2021, Sustainability of Parliament and of the Council and the implementation of
construction works — Environmental Product Declarations — specific objectives set out in Commission Delegated Decision
Core rules for the product category of construction products. (EU) 2017/1474
COMMISSION IMPLEMENTING REGULATION (EU) 2020/387
of 9 March 2020 amending Regulations (EU) No 321/2013,
Further References (EU) No 1302/2014 and (EU) 2016/919 as regards the
extension of the area of use and transition phases
GaBi Software/Database Candidate List of substances of very high concern for
GaBi Software System and Database for Life Cycle Authorisation (published in accordance with Article 59(10) of
Engineering, Sphera Solution GmbH, Leinfelden-Echterdingen, the REACH Regulation)
2022 (https://www.gabi-software.com/support/gabi)
https://echa.europa.eu/de/candidate-list-table
IBU 2023 REGULATION (EU) No 528/2012 OF THE EUROPEAN
Institut Bauen und Umwelt e.V.: General Instructions for the PARLIAMENT AND OF THE COUNCIL of 22 May 2012
EPD programme of Institut Bauen und Umwelt e.V., Version concerning the making available on the market and use of
2.0, Berlin: Institut Bauen und Umwelt e.V., 2023, www.ibu- biocidal products
epd.com
5 Environmental Product Declaration - Saarstahl Rail - Pure Steel+ Rail
Publisher
Institut Bauen und Umwelt e.V. +49 (0)30 3087748- 0
Hegelplatz 1 info@ibu-epd.com
10117 Berlin www.ibu-epd.com
Germany
Programme holder
Institut Bauen und Umwelt e.V. +49 (0)30 3087748- 0
Hegelplatz 1 info@ibu-epd.com
10117 Berlin www.ibu-epd.com
Germany
Author of the Life Cycle Assessment
Sphera Solutions GmbH +49 (0)711 341817-0
Hauptstraße 111- 113 info@sphera.com
70771 Leinfelden-Echterdingen www.sphera.com
Germany
Owner of the Declaration
Saarstahl Rail +33382574500
Rue du Maréchal Foch 164 contact@saarstahl-rail.fr
57705 Hayange Cedex www.saarstahl-rail.fr
France
6 Environmental Product Declaration - Saarstahl Rail - Pure Steel+ Rail
