ENVIRONMENTAL PRODUCT DECLARATION
as per ISO 14025 and EN 15804+A2
Owner of the Declaration dormakaba International Holding GmbH
Publisher Institut Bauen und Umwelt e.V. (IBU)
Programme holder Institut Bauen und Umwelt e.V. (IBU)
Declaration number EPD-DOR-20240088-CBA1-EN
Issue date 14.03.2024
Valid to 18.10.2027
Door closer TS 92 Contur
dormakaba
www.ibu-epd.com | https://epd-online.com
General Information
dormakaba Door closer TS 92 Contur
Programme holder Owner of the declaration
IBU – Institut Bauen und Umwelt e.V. dormakaba International Holding GmbH
Hegelplatz 1 DORMA Platz 1
10117 Berlin 58256 Ennepetal
Germany Germany
Declaration number Declared product / declared unit
EPD-DOR-20240088-CBA1-EN 1 door closer (1 piece) of the TS 92 Contur
This declaration is based on the product category rules: Scope:
Building Hardware products, 01.08.2021 This Environmental Product Declaration refers to a specific door closer
(PCR checked and approved by the SVR) manufactured by dormakaba Production GmbH & CO KG. The production
site is located in Singapore.
Issue date The data represents the year 2020.
The owner of the declaration shall be liable for the underlying information
14.03.2024
and evidence; the IBU shall not be liable with respect to manufacturer
information, life cycle assessment data and evidences.
Valid to
The EPD was created according to the specifications of EN 15804+A2. In
18.10.2027 the following, the standard will be simplified as EN 15804.
Verification
The standard EN 15804 serves as the core PCR
Independent verification of the declaration and data according to ISO
14025:2011
internally X externally
Dipl.-Ing. Hans Peters
(Chairman of Institut Bauen und Umwelt e.V.)
Florian Pronold Dr.-Ing. Wolfram Trinius,
(Managing Director Institut Bauen und Umwelt e.V.) (Independent verifier)
1 Environmental Product Declaration - dormakaba - Door closer TS 92 Contur
Product
Performance data of the product with respect to its
Product description/Product definition characteristics in accordance with the relevant technical
The universal slide channel door closer for standard doors provision which can be applied are mentioned above.
features EASY OPEN technology for easy door opening. The
TS 92 Contur slide channel door closer is an attractive and Base materials/Ancillary materials
competitively priced complement to the TS 98 XEA range. The major material compositions including the packaging of the
For the use and application of the product the respective product are listed below:
national provisions at the place of use apply. The standards Name Value Unit
which can be applied are the following:
Steel 38 %
• EN 1154 Aluminium 37 %
• EN 1634-1
Paper 14 %
Application Zinc 4 %
It can be used for any interior application. Lubricants 4 %
Plastics 2 %
Technical Data
Others 1 %
The door closer has following technical properties:
The product includes partial articles which contain substances
listed in the Candidate List of REACH Regulation
1907/2006/EC (date: 23.01.2024) exceeding 0.1 percentage by
mass: yes
• Lead (Pb): 7439-92-1 (CAS-No.) is included in some of
the alloys used. The concentration of lead in each
individual alloy does not exceed 4.0% (by mass).
The Candidate List can be found on the ECHA website
address: https:echa.europa.eu/de/home.
Reference service life
The reference service life of the TS 92 Contur door closer
depends on the traffic pattern and degree of usage of the door.
These closers are rated to EN 1154, meaning they are
designed to withstand a minimum of 500,000 cycles. The
reference service life amounts for 20 years. This corresponds
with approx. 25,000 cycles per year.
LCA: Calculation rules
The product stage includes:
Declared Unit — A1, raw material extraction, processing and
The declared unit is 1 piece of the product: TS 92 Contur. mechanical treatments, processing of secondary
Name Value Unit material input (e.g. recycling processes),
Declared unit 1 piece/product — A2, transport to the manufacturer,
— A3, manufacturing and assembly
Mass of declared Product 3.34 kg
including provision of all materials, products and energy, as well
as waste processing up to the end-of waste state.
System boundary
The type of EPD is: cradle to gate with options,
Construction stage - Modules A4-A5
modules C1–C4, and module D
The construction process stage includes:
(A1–A3 + C + D and additional modules: A4 + A5)
— A4, transport to the building site;
— A5, installation into the building;
Production - Module A1-A3
including provision of all materials, products and energy, as well
2 Environmental Product Declaration - dormakaba - Door closer TS 92 Contur
as waste processing up to the end-of waste state or disposal of and benefits.
final residues during the construction process stage.
Geographic Representativeness
End-of-life stage– Modules C1-C4 and D Land or region, in which the declared product system is
The end-of-life stage includes: manufactured, used or handled at the end of the product´s
— C1, de-construction, demolition: lifespan: Global
— C2, transport to waste processing;
— C3, waste processing for reuse, recovery and/or
Comparability
recycling;
Basically, a comparison or an evaluation of EPD data is only
— C4, disposal;
possible if all the data sets to be compared were created
including provision and all transport, provision of all
according to EN 15804 and the building context, respectively
materials, products and related energy and water use.
the product-specific characteristics of performance, are taken
Module D (Benefits and loads beyond the system
into account.
boundary) includes:
— D, recycling potentials, expressed as net impacts
LCA: Scenarios and additional technical information
Installation into the building (A5)
Characteristic product properties of biogenic carbon
Name ValueUnit
Name ValueUnit
Output substances following waste treatment on
kg 0.06 kg
Biogenic carbon content in product 0.15 site (packaging)
C
Biogenic carbon content in accompanying 0.02 kg End of life (C1-C4)
packaging C
C1: The product dismantling from the building is done manually
without environmental burden.
C2: Transport to waste treatment at end of life is 50 km.
Transport to the building site (A4) Name Value Unit
Name Value Unit Collected separately waste type waste type 3.28 kg
Litres of fuel truck (per piece) 0.00276l/100km Recycling 3.22 kg
Transport distance via truck (from habor to Energy recovery 0.059 kg
300 km
dormakaba logistic center) Final disposal 0,13 kg
Transport distance via truck (for scaling) 100 km
Reuse, recovery and/or recycling potentials (D), relevant
Capacity utilisation (including empty runs)
55 % scenario information
average
Name Value Unit
Transport distance via ship 11000 km
Recycling 100 %
The product is transported via truck and ship. The product is
Collection rate is 100%.
stored in the dormakaba logistic center in Germany. The main
distribution region is Europe. In order to allow scaling to a
specific point of installation 100 km are declared as well.
3 Environmental Product Declaration - dormakaba - Door closer TS 92 Contur
LCA: Results
DESCRIPTION OF THE SYSTEM BOUNDARY (X = INCLUDED IN LCA; MND = MODULE OR INDICATOR NOT DECLARED; MNR
= MODULE NOT RELEVANT)
Benefits and
Construction loads beyond
Product stage Use stage End of life stage
process stage the system
boundaries
la ire ta m w a Ry lp p u s tro p s n a rT g n iru tc a fu n a M e h t m o rf tro p s n a rTe tis e h t o t e ta g y lb m e s s A e s U e c n a n e tn ia M ria p e R tn e m e c a lp e R tn e m h s ib ru fe R y g re n e la n o ita re p Oe s u re ta w la n o ita re p Oe s u n o itc u rts n o c -e Dn o itilo m e d tro p s n a rT g n is s e c o rp e ts a W la s o p s iD -e s u e R-y re v o c e R-g n ilc y c e Rla itn e to p
A1 A2 A3 A4 A5 B1 B2 B3 B4 B5 B6 B7 C1 C2 C3 C4 D
X X X X X MND MND MNR MNR MNR MND MND X X X X X
RESULTS OF THE LCA - ENVIRONMENTAL IMPACT according to EN 15804+A2: 1 door closer
Parameter Unit A1-A3 A4 A5 C1 C2 C3 C4 D
GWP-total kg CO 2 eq 2.52E+01 2.37E-01 8.5E-02 0 1.4E-02 1.29E+00 0 -9.03E+00
GWP-fossil kg CO 2 eq 2.59E+01 2.32E-01 2E-03 0 1.4E-02 5.62E-01 0 -9E+00
GWP-biogenic kg CO 2 eq -7.44E-01 5E-03 8.3E-02 0 6.32E-04 7.31E-01 0 -2.8E-02
GWP-luluc kg CO 2 eq 9E-03 5.13E-06 1.4E-06 0 3.25E-07 3.83E-05 0 -2E-03
ODP kg CFC11 eq 8.97E-11 2.31E-17 1.53E-17 0 1.44E-18 3.68E-16 0 -6.19E-11
AP mol H+ eq 1.29E-01 5E-03 2.38E-05 0 1.37E-05 2.04E-04 0 -3.3E-02
EP-freshwater kg P eq 2.48E-05 5.1E-08 3E-09 0 2.93E-09 5.78E-08 0 -5.87E-06
EP-marine kg N eq 2.06E-02 1E-03 8.6E-06 0 4.35E-06 5.67E-05 0 -4E-03
EP-terrestrial mol N eq 2.19E-01 1.3E-02 1.07E-04 0 4.84E-05 9.48E-04 0 -4.8E-02
kg NMVOC
POCP 6.3E-02 3E-03 2.28E-05 0 1.23E-05 1.55E-04 0 -1.4E-02
eq
ADPE kg Sb eq 6.16E-04 6.44E-09 2.42E-10 0 4.1E-10 5.25E-09 0 -1.93E-04
ADPF MJ 2.81E+02 3.04E+00 2.7E-02 0 1.94E-01 4.15E-01 0 -1.27E+02
m3 world eq
WDP 3.9E+00 4.35E-04 1.1E-02 0 2.68E-05 1.33E-01 0 -5.04E-01
deprived
GWP = Global warming potential; ODP = Depletion potential of the stratospheric ozone layer; AP = Acidification potential of land and water; EP =
Eutrophication potential; POCP = Formation potential of tropospheric ozone photochemical oxidants; ADPE = Abiotic depletion potential for non-fossil
resources; ADPF = Abiotic depletion potential for fossil resources; WDP = Water (user) deprivation potential)
RESULTS OF THE LCA - INDICATORS TO DESCRIBE RESOURCE USE according to EN 15804+A2: 1 door closer
Parameter Unit A1-A3 A4 A5 C1 C2 C3 C4 D
PERE MJ 5.39E+01 1E-02 7.25E-01 0 6.11E-04 4.99E+00 0 -5.49E+01
PERM MJ 5.61E+00 0 -7.2E-01 0 0 -4.89E+00 0 0
PERT MJ 5.95E+01 1E-02 5E-03 0 6.11E-04 9.6E-02 0 -5.49E+01
PENRE MJ 2.79E+02 3.04E+00 2.7E-02 0 1.94E-01 2.43E+00 0 -1.27E+02
PENRM MJ 2.02E+00 0 0 0 0 -2.02E+00 0 0
PENRT MJ 2.81E+02 3.04E+00 2.7E-02 0 1.94E-01 4.15E-01 0 -1.27E+02
SM kg 9.8E-01 0 0 0 0 0 0 0
RSF MJ 0 0 0 0 0 0 0 0
NRSF MJ 0 0 0 0 0 0 0 0
FW m3 1.48E-01 1.76E-05 2.48E-04 0 1.1E-06 3E-03 0 -9.7E-02
PERE = Use of renewable primary energy excluding renewable primary energy resources used as raw materials; PERM = Use of renewable primary
energy resources used as raw materials; PERT = Total use of renewable primary energy resources; PENRE = Use of non-renewable primary energy
excluding non-renewable primary energy resources used as raw materials; PENRM = Use of non-renewable primary energy resources used as raw
materials; PENRT = Total use of non-renewable primary energy resources; SM = Use of secondary material; RSF = Use of renewable secondary fuels;
NRSF = Use of non-renewable secondary fuels; FW = Use of net fresh water
RESULTS OF THE LCA – WASTE CATEGORIES AND OUTPUT FLOWS according to EN 15804+A2:
1 door closer
Parameter Unit A1-A3 A4 A5 C1 C2 C3 C4 D
HWD kg 3.42E-06 2.97E-10 3.96E-11 0 1.88E-11 1.09E-09 0 -9.5E-07
NHWD kg 4.26E+00 3.11E-04 3E-03 0 1.98E-05 6.3E-02 0 -1.99E+00
RWD kg 6.74E-03 3.32E-06 1.41E-06 0 2.08E-07 1.86E-05 0 -1.3E-02
CRU kg 0 0 0 0 0 0 0 0
MFR kg 0 0 0 0 0 2.65E+00 0 0
MER kg 0 0 0 0 0 0 0 0
EEE MJ 0 0 1.29E-01 0 0 0 0 0
EET MJ 0 0 2.33E-01 0 0 0 0 0
HWD = Hazardous waste disposed; NHWD = Non-hazardous waste disposed; RWD = Radioactive waste disposed; CRU = Components for re-use;
MFR = Materials for recycling; MER = Materials for energy recovery; EEE = Exported electrical energy; EET = Exported thermal energy
4 Environmental Product Declaration - dormakaba - Door closer TS 92 Contur
RESULTS OF THE LCA – additional impact categories according to EN 15804+A2-optional:
1 door closer
Parameter Unit A1-A3 A4 A5 C1 C2 C3 C4 D
Disease
PM 3.13E-06 7.62E-08 1.32E-10 0 7.19E-11 1.79E-09 0 -5.18E-07
incidence
IR kBq U235 eq 1.05E+00 4.77E-04 2.18E-04 0 2.98E-05 2E-03 0 -2.63E+00
ETP-fw CTUe 9.59E+01 2.15E+00 1.3E-02 0 1.37E-01 1.65E-01 0 -4.53E+01
HTP-c CTUh 1.22E-08 4.05E-11 6.74E-13 0 2.58E-12 1.29E-11 0 -1.65E-10
HTP-nc CTUh 3.5E-07 1.82E-09 2.92E-11 0 1.11E-10 1E-09 0 1.36E-07
SQP SQP 1.07E+02 8E-03 7E-03 0 4.98E-04 1.21E-01 0 -4.35E+00
PM = Potential incidence of disease due to PM emissions; IR = Potential Human exposure efficiency relative to U235; ETP-fw = Potential comparative
Toxic Unit for ecosystems; HTP-c = Potential comparative Toxic Unit for humans (cancerogenic); HTP-nc = Potential comparative Toxic Unit for humans
(not cancerogenic); SQP = Potential soil quality index
Disclaimer 1 – for the indicator “Potential Human exposure efficiency relative to U235”. This impact category deals mainly with the
eventual impact of low-dose ionizing radiation on human health of the nuclear fuel cycle. It does not consider effects due to possible
nuclear accidents, occupational exposure or radioactive waste disposal in underground facilities. Potential ionizing radiation from the
soil, radon and from some construction materials is also not measured by this indicator.
Disclaimer 2 – for the indicators “abiotic depletion potential for non-fossil resources”, “abiotic depletion potential for fossil resources”,
“water (user) deprivation potential, deprivation-weighted water consumption”, “potential comparative toxic unit for ecosystems”,
“potential comparative toxic unit for humans – cancerogenic”, “Potential comparative toxic unit for humans - not cancerogenic”,
“potential soil quality index”. The results of this environmental impact indicator shall be used with care as the uncertainties on these
results are high as there is limited experience with the indicator.
References
EN 1154 GaBi
EN 1154-2003; Building hardware - Controlled door closing Sphera Solutions GmbH
devices - Requirements and test methods Gabi Software System and Database for Life Cycle
Engineering 1992-2020
EN 1634-1 Version 10.0.0.71
EN 1634-1:2018; Fire resistance and smoke control tests for University of Stuttgart
door and shutter assemblies, openable windows and elements Leinfelden-Echterdingen
of building hardware - Part 1: Fire resistance test for door and
shutter assemblies and openable windows GaBi ts documentation
GaBi life cycle inventory data documentation (https://www.gabi-
ISO 14025 software.com/support/gabi/gabidatabase-2020-lci-
DIN EN ISO 14025:2011-10, Environmental labels and documentation/)
declarations — Type III environmental declarations —
Principles and procedures LCA-tool dormakaba
LCA-tool, IBU-DOR-202104-LT1-EN, 2021,
EN 15804 developed by Sphera Solutions GmbH
EN 15804+A2:2019+AC:2021, Sustainability of construction
works — Environmental Product Declarations — Core rules for PCR Part A
the product category of construction products PCR – Part A: Calculation Rules for the Life Cycle Assessment
and Requirements on the Project Report according to EN
REACH Regulation 15804+A2:2019, Version 1.0, 2020, Institut Bauen und Umwelt
Regulation (EC) No 1907/2006 of the European Parliament and e.V., www.ibu-epd.com
of the Council on the Registration, Evaluation, Authorisation
and Restriction of Chemicals (REACH) PCR Part B
PCR – Part B: Requirements on the EPD for Building Hardware
Further References product, version 1.2, Institut Bauen und Umwelt e.V., www.ibu-
epd.com, 2017
IBU 2021
General Instructions for the EPD programme of InstitutBauen
und Umwelt e.V. Version 2.0, Berlin: InstitutBauen und Umwelt
e.V., 2021. www.ibu-epd.com
5 Environmental Product Declaration - dormakaba - Door closer TS 92 Contur
Publisher
Institut Bauen und Umwelt e.V. +49 (0)30 3087748- 0
Hegelplatz 1 info@ibu-epd.com
10117 Berlin www.ibu-epd.com
Germany
Programme holder
Institut Bauen und Umwelt e.V. +49 (0)30 3087748- 0
Hegelplatz 1 info@ibu-epd.com
10117 Berlin www.ibu-epd.com
Germany
Author of the Life Cycle Assessment
dormakaba International Holding GmbH +49 2333 793-0
DORMA Platz 1 info.de@dormakaba.com
58256 Ennepetal www.dormakaba.com
Germany
Owner of the Declaration
dormakaba International Holding GmbH +49 2333 793-0
DORMA Platz 1 info.de@dormakaba.com
58256 Ennepetal www.dormakaba.com
Germany
6 Environmental Product Declaration - dormakaba - Door closer TS 92 Contur
