ENVIRONMENTAL PRODUCT DECLARATION
as per ISO 14025 and EN 15804+A2
Owner of the Declaration Rubner Holding AG - S.p.A.
Publisher Institut Bauen und Umwelt e.V. (IBU)
Programme holder Institut Bauen und Umwelt e.V. (IBU)
Declaration number EPD-RUB-20230228-IBC1-EN
Issue date 27.06.2023
Valid to 26.06.2028
Rubner Sawn Timber, Rubner Sawn Timber kiln dried, Rubner
Sawn Timber machine graded
Rubner Holding AG - S.p.A
www.ibu-epd.com | https://epd-online.com
1. General Information
Rubner Holding AG - S.p.A Rubner Sawn Timber, Rubner Sawn Timber kiln
dried, Rubner Sawn Timber machine graded
Programme holder Owner of the declaration
IBU – Institut Bauen und Umwelt e.V. Rubner Holding AG - S.p.A.
Hegelplatz 1 Handwerkerzone 2
10117 Berlin 39030 Kiens
Germany Italy
Declaration number Declared product / declared unit
EPD-RUB-20230228-IBC1-EN 1 m³ of kiln dried, planed, machine graded sawn timber [ST] with an
average density of 459 kg/m³
This declaration is based on the product category rules: Scope:
Solid wood products, 01.08.2021 This EPD is based on a declared unit of 1 m³ of kiln dried, planed, machine
(PCR checked and approved by the SVR) graded sawn timber (moisture of 12 % at a raw density of 459 kg/m³)
produced at the RUBNER production site in Rohrbach (Austria).
Issue date The owner of the declaration shall be liable for the underlying information
and evidence; the IBU shall not be liable with respect to manufacturer
27.06.2023
information, life cycle assessment data and evidences.
The EPD was created according to the specifications of EN 15804+A2. In
Valid to
the following, the standard will be simplified as EN 15804.
26.06.2028
Verification
The standard EN 15804 serves as the core PCR
Independent verification of the declaration and data according to ISO
14025:2011
internally X externally
Dipl.-Ing. Hans Peters
(Chairman of Institut Bauen und Umwelt e.V.)
Dipl.-Ing. Hans Peters Matthias Schulz,
(Managing Director Institut Bauen und Umwelt e.V.) (Independent verifier)
1 Environmental Product Declaration - Rubner Holding AG - S.p.A - Rubner Sawn Timber, Rubner Sawn Timber kiln dried, Rubner Sawn Timber machine graded
2. Product
Constructional data
2.1 Product description/Product definition
RUBNER sawn timber is produced from fresh roundwood, Name Value Unit
whereby the wood species spruce and pine are processed in spruce, pine,
Wood types by trade names acc. to EN
accordance with EN 1912 (Picea abies and Pinus sylvestris). larch, -
1912
The roundwood for the production of RUBNER sawnwood Douglas fir
originates from a predominantly regional supply network, the Wood moisture acc. to EN 13183-1 < 18 %
average delivery distance of the roundwood is around 80 km.
Use of wood preservatives (the wood
Depending on the processing level, RUBNER sawn timber is
preservative test mark to DIN 68800-3 n.r. -
available as fresh, dried, dried/pre-planed or
must be indicated)
dried/planed/(visually) machine-graded lath, board or plank
Compressive strength parallel acc. to EN
sawn timber. In the manufacturing process, prismatic timber 16 - 30 N/mm2
1995
pieces are cut from the logs in a first processing step, whereby
the dimensions produced are essentially in conformity with the Compressive strength rectangular acc. to 2 - 3 N/mm2
specifications according to DIN 4074-1. The individual pieces, EN 1995
RUBNER sawn timber, always have a fibre direction parallel to Tensile strength parallel acc. to EN 1995 8 - 30 N/mm2
the longitudinal axis. Subsequently, kiln drying takes place, Tensile strength rectangular acc. to EN
optionally in drying chambers or drying channels. The kiln-dried 1995
0.4 N/mm2
RUBNER sawn timber is then forwarded for further processing
7000 -
in the form of planing or pre-planing/grading. In the course of Modulus of elasticity acc. to EN 1995 N/mm2
16000
timber grading, the pre-planed sawn timber is classified
Shear strength acc. to EN 1995 2.5 - 4 N/mm2
according to visual and mechanical strength and stiffness
properties. Shear modulus acc. to EN 1995 440 - 970 N/mm2
For visual grading, the specifications according to DIN 4074-1 Dimensional deviation acc. EN 336 Class 2 mm
apply, whereby the grading classes (S7-S13) are assigned to
Length (min. - max.) 2 - 5 m
the European strength classes (EN 338) on the basis of EN
Width (min. - max.) 0.08 - 0.35 m
1912.
For machine strength grading, the specifications according to Height (min. - max.) 0.01 - 0.1 m
EN 14081 (all parts) apply. RUBNER sawn timber is almost Gross density supporting components in
completely graded by machine (98 %), only in exceptional accordance with EN 338 or DIN 1052.
350-520 kg/m3
cases is it visually graded using equipment. Non-supporting components are
Due to the kiln drying combined with the machine grading, classified as per DIN 68364
RUBNER sawn timber has good dimensional stability and Surface quality (Possible characteristic rough sawn,
-
reduced cracking behaviour. features must be indicated) planed
For the placing on the market of the product in the European
Risk class acc. to 68800-3 5 -
Union/European Free Trade Association (EU/EFTA) (with the
Thermal conductivity acc. to EN 12664 0.12 W/mK
exception of Switzerland) Regulation (EU) No. 305/2011 CPR
Specific heat capacity acc. to EN 12664 1.6 kJ/kgK
applies. The product meets the requirements of EN 15497 and
the CE-marking. For use, the respective national regulations Water vapor diffusion equivalent air layer
n.r m
apply. thickness acc. to ISO 12572
Water vapour diffusion resistance factor
2.2 Application 20-50 -
acc. to ISO 12572
RUBNER sawn timber classified according to purely visual
Formaldehyde emissions acc. to EN
criteria is used in the construction sector for both decorative n.r. μg/m3
14081
and structural purposes.
RUBNER sawn timber graded according to its strength can be The essential properties and performance characteristics of
used for the construction of load-bearing components in RUBNER sawn timber comply with the requirements of EN
buildings and bridges. RUBNER sawn timber graded according 14081-1:2005+A1(2011).
to its strength is mainly used as a base material for various
2.4 Delivery status
wood-based materials such as glulam, cross-laminated timber
RUBNER sawn timber is produced with the dimensions
or finger-jointed solid structural timber.
according to chapter 2.3 and is delivered in domestic visual
quality, visual quality or industrial quality. The tolerances
2.3 Technical Data according to EN 336 are met.
RUBNER sawn timber has the mechanical properties required
2.5 Base materials/Ancillary materials
for use in timber structures according to EN 1995 (all parts).
RUBNER sawn timber comprises kiln-dried coniferous
The following technical data apply to the properties of RUBNER
structural timber with rectangular cross sections. (Picea abies
sawn timber. The performance data of the product are in
and Pinus sylvestris), whereby no auxiliary substances and
accordance with its essential characteristics according to EN
additives are used.
14081.
The product has an average density of 459 kg/m³.
This product/article/at least one partial article contains
substances listed in the candidate list (date: 17.01.2023)
exceeding 0.1 percentage by mass: no.
2 Environmental Product Declaration - Rubner Holding AG - S.p.A - Rubner Sawn Timber, Rubner Sawn Timber kiln dried, Rubner Sawn Timber machine graded
This product/article/at least one partial article contains other Health protection: Under normal conditions of use, RUBNER
carcinogenic, mutagenic, reprotoxic (CMR) substances in sawn timber is not expected to cause any damage or
categories 1A or 1B which are not on the candidate list, impairments to health.
exceeding 0.1 percentage by mass: no.
2.12 Reference service life
Biocide products were added to this construction product or it For structural applications, the reference service life according
has been treated with biocide products (this then concerns a to ISO 15686 is at least 50 years. When used as designated,
treated product as defined by the (EU) Ordinance on Biocide no end of durability must be expected due to its natural
Products No. 528/2012): no. durability (protection against moisture). When used as
designated, the lifetime of RUBNER sawn timber is equal to the
2.6 Manufacture duration of use of the building. For structural applications, the
RUBNER sawn timber is manufactured from sustainable wood reference service life according to ISO 15686 is at least 50
(PEFC) sourced from sustainable forestry. After delivery to the years.
production facility, a quality and volume assessment is carried The values quoted are based on empirical values and require
out. After debarking, the logs are classified according to their strict compliance with the requirements of EN 1995-1-1 (service
diameter and temporarily stored at the log yard (dry & wet classes) combined with periodic inspection and maintenance.
storage). In the sawing line, the logs are split into main and The values do not represent warranty periods from which
sideboards with circular saws and then (sideboards) warranty claims can be derived.
prismatically edged.
RUBNER sawn timber that is not dried is then visually graded
and packaged. 2.13 Extraordinary effects
Dried RUBNER sawn timber is kiln dried after the sawing Fire
process, with a target moisture content between 10 and For RUBNER sawn timber, the following applies regarding the
18 percent. fire behaviour according to EN 13501-1.
RUBNER sawn timber graded according to strength is pre- Fire protection
planed after technical drying and then visually or mechanically
Name Value
graded by strength.
Building material class D
Optionally, the kiln-dried Rubner sawn timber is protected from
the weather during intermediate storage and transport with Burning droplets d0
foils. Smoke gas development s2
2.7 Environment and health during manufacturing
Water
During production, there are no negative impacts on water and
No ingredients are washed out which could be hazardous to
soil. The resulting process wastewater is fed into the local
water.
sewage system and cleaned according to legal regulations. The
resulting exhaust air is cleaned according to legal regulations.
Mechanical destruction
Noise emissions from industrial plants are reduced by structural
The fracture behaviour of RUBNER sawn timber is appearance
measures and comply with the legal requirements.
typical for solid wood.
The employee protection in the manufacturing process
complies with the respective country-specific requirements,
2.14 Re-use phase
employees are provided with personal protective equipment.
In the event of selective de-construction, RUBNER sawn timber
2.8 Product processing/Installation can easily be re-used after the end of the structure's service
life.
RUBNER sawn timber can be processed with commercially
The preferred use of RUBNER sawn timber is in the form of
available tools. The instructions for occupational
reuse based on the applicable country-specific requirements.
safety/assembly are to be observed.
If it is not reused, it will be subjected to thermal utilization for
2.9 Packaging the production of heat and electricity due to the high calorific
Polyethylene foils are used in small quantities during value of approx. 16.5 MJ/kg (at a humidity of u = 12 %) in
transportation. compliance with the applicable country-specific requirements.
2.10 Condition of use 2.15 Disposal
The composition of RUBNER sawn timber corresponds to the If the residues are not used for any other cascading use, waste
composition according to Section 2.5 for the entire period of wood is disposed according to the applicable country-specific
use. requirements. Disposal represents a possible but unusual case.
RUBNER sawn timber is assigned to waste code 17 02 01 in
2.11 Environment and health during use the European list of waste 2014/955/EU.
Environmental protection: According to current knowledge, the
2.16 Further information
intended use of RUBNER sawn timber does not present any
hazards or impairments to water, air and soil. More detailed information is available at: www.rubner.com
3. LCA: Calculation rules
Declared unit
3.1 Declared Unit
This EPD refers to a declared unit of 1 m³ of sawn timber Name Value Unit
produced by the RUBNER group. The declared unit refers to an Declared unit 1 m3
average density of 459 kg/m³ and wood moisture at delivery of Gross density 459 kg/m3
12 %.
Wood moisture at delivery 12 %
3 Environmental Product Declaration - Rubner Holding AG - S.p.A - Rubner Sawn Timber, Rubner Sawn Timber kiln dried, Rubner Sawn Timber machine graded
The analysed products represent average sawn timber market whenever European or regionalised average data were
produced at the RUBNER site in Rohrbach (AT). not available.
The declared unit was calculated on a volume-weighted basis. Emissions from wood drying were included in the calculations
This EPD refers to an average product manufactured at one according to Rüter & Diederichs 2012.
site. All products undergo the same processing steps. A
possible variability is only expected due to the use of different 3.4 Cut-off criteria
wood species. The upstream chain for spruce is considered The LCA model covers all available input and output flows,
representative. The robustness of the declared LCA values can which can be represented based on robust data and from which
thus be classified as high. a significant contribution can be expected. Data gaps are filled
with conservative assumptions of average data or generic data
if available and are documented accordingly.
Only data with a contribution of less than 1 % were cut off.
3.2 System boundary Thus, no data were neglected, of which a substantial impact is
The life cycle assessment of average sawn timber produced by to be expected. All relevant data were collected
RUBNER refers to a cradle-to-gate analysis of the comprehensively. Cutoff material and energy flows were
environmental impacts with modules C1–C4 and module D chosen carefully based on their expected quantitative
(A1–A3 + C + D). The following life cycle phases are part of the contribution as well as potential environmental impacts. Thus, it
analysis: can be assumed that the sum of all neglected input flows does
not account for more than 5 % of the total material, water and
Module A1–A3 | Production stage energy flows. Environmental impacts of machines, plant and
The production stage includes the upstream burdens of raw infrastructure were not included.
materials (round timber, etc.) and the corresponding transports
to the RUBNER production site in Rohrbach (Austria). Direct 3.5 Background data
emissions from drying are based on worst-case approximations This study uses generic background data for the evaluation of
and are included in the study. RUBNER produces thermal upstream environmental impacts from GaBi database 2022.2
energy in its own biomass boilers. Electricity is provided by the as well as recognised literature such as Rüter & Diederichs
own photovoltaic system as well as 100 % green electricity. 2012.
3.6 Data quality
Module C1 | Deconstruction and demolition
After the removal of building components overlying the product, Data collection is based on product-specific questionnaires. It
the joints can simply be loosened by screwing or sawing and follows an iterative process of clarifying questions via e-mail,
lifted by cranes to the place of removal. Required energy telephone calls or in personal/web meetings. Intensive
demand can be neglected. The actual energy demand depends discussions between the RUBNER group and Daxner & Merl
on the installation of the products and can therefore vary result in an accurate mapping of product-related material and
greatly in the building context. energy flows. This leads to a high quality of foreground data
collected. Data collection relies on a consistent process
Module C2 | Transport to disposal according to ISO 14044.
Module C2 includes the transport to waste treatment. In this
case, transport by truck over a transport distance of 50 km is The technological, geographical and time-related
assumed. representativeness of the database was kept in mind when
selecting background data. Whenever specific data were
Module C3 | Waste processing missing, either generic datasets or representative average data
In Module C3, the chipping after removal of the products is were used instead. The implemented GaBi background
considered. The wooden products and with them the material- datasets refer to the latest versions available and are carefully
inherent properties leave the product system as secondary chosen.
combustibles in module C3.
The assessment of the robustness of the average can be found
Module C4 | Disposal in Section 3.1.
The applied scenario declares the energetic recovery of the
3.7 Period under review
wooden products, therefore no environmental impacts are to be
Foreground data were collected in the 2022 production year,
expected from the waste processing of the products in C4.
and the data are based on the volumes produced on annual
basis.
Module D | Benefits and loads beyond the system
boundary
3.8 Geographic Representativeness
Applying an European average scenario, module D describes
Land or region, in which the declared product system is
the energetic recovery of the product at the end of life including
manufactured, used or handled at the end of the product´s
the corresponding energy substitution potentials.
lifespan: Austria
3.3 Estimates and assumptions
All assumptions are verified through detailed documentation 3.9 Allocation
and correspond to the best possible representation of reality
The carbon content and primary energy content of the products
based on the available data. Background data for wood logs
were assessed based on their material inherent properties
refer to generic data for spruce logs in bark derived from GaBi
according to underlying physical relationships.
database. Spruce represents the majority of wood processed at
RUBNER. The used dataset represents an approximation for all 3.10 Comparability
other species. Basically, a comparison or an evaluation of EPD data is only
Regional applicability of the used background data refers to possible if all the data sets to be compared were created
average data under European or German conditions taken from according to EN 15804 and the building context, respectively
the GaBi database. German data were used for the Austrian the product-specific characteristics of performance, are taken
4 Environmental Product Declaration - Rubner Holding AG - S.p.A - Rubner Sawn Timber, Rubner Sawn Timber kiln dried, Rubner Sawn Timber machine graded
into account. The GaBi background database was used to calculate the LCA
(GaBi 10; 2022.2).
4. LCA: Scenarios and additional technical information
Reuse, recovery and/or recycling potentials (D), relevant
Characteristic product properties of biogenic carbon
scenario information
During tree growth, the wood assimilates carbon dioxide and
stores biogenic carbon. The carbon stored in the product is Name Value Unit
declared in the following table. Processing rate 100 %
Information on describing the biogenic carbon content at Efficiency of power plant 68 %
factory gate The product reaches the end-of-waste status after removal from
Name Value Unit the building, transport to processing and chipping of the
Biogenic carbon content in product 205 kg C product. For the end of life of the sawn timber product, energy
recovery as secondary fuel in a biomass power plant is
The product is delivered without packaging. Minor quantities
assumed. As the main sales market for the solid wood products
optionally used were neglected.
is concentrated in the European region, plant-specific
characteristic values correspond to a European average
scenario (EU). The scenario considers a reprocessing rate of
100 % for solid wood products after removal from the building.
This assumption has to be adjusted accordingly when applying
the results in the building context. At the end of life of the
End of life (C1-C4) product, the equilibrium moisture is comparable to the moisture
Name Value Unit content at delivery. This value can vary depending on the
storage of the product before energy recovery.
Energy recovery 459 kg
5 Environmental Product Declaration - Rubner Holding AG - S.p.A - Rubner Sawn Timber, Rubner Sawn Timber kiln dried, Rubner Sawn Timber machine graded
5. LCA: Results
The following table contains the LCA results for a declared unit of 1 m³ of sawn timber produced by the RUBNER group (459 kg/m³).
DESCRIPTION OF THE SYSTEM BOUNDARY (X = INCLUDED IN LCA; ND = MODULE OR INDICATOR NOT DECLARED; MNR =
MODULE NOT RELEVANT)
Benefits and
Construction loads beyond
Product stage Use stage End-of-life stage
process stage the system
boundaries
la ire ta m w a Ry lp p u s tro p s n a rT g n iru tc a fu n a M e h t m o rf tro p s n a rTe tis e h t o t e ta g y lb m e s s A e s U e c n a n e tn ia M ria p e R tn e m e c a lp e R tn e m h s ib ru fe R y g re n e la n o ita re p Oe s u re ta w la n o ita re p Oe s u n o itc u rts n o c -e Dn o itilo m e d tro p s n a rT g n is s e c o rp e ts a W la s o p s iD -e s u e R-y re v o c e R-g n ilc y c e Rla itn e to p
A1 A2 A3 A4 A5 B1 B2 B3 B4 B5 B6 B7 C1 C2 C3 C4 D
X X X MND MND MND MND MNR MNR MNR MND MND X X X X X
RESULTS OF THE LCA - ENVIRONMENTAL IMPACT according to EN 15804+A2: 1 m³ sawn timber (459 kg/m³)
Parameter Unit A1-A3 C1 C2 C3 C4 D
Global Warming Potential total (GWP-total) kg CO 2 eq -7.27E+02 0 1.45E+00 7.62E+02 0 -4.1E+02
Global Warming Potential fossil fuels (GWP-fossil) kg CO 2 eq 2.85E+01 0 1.38E+00 3.39E+00 0 -3.81E+02
Global Warming Potential biogenic (GWP-biogenic) kg CO 2 eq -7.56E+02 0 6.02E-02 7.58E+02 0 -2.92E+01
Global Warming Potential luluc (GWP-luluc) kg CO 2 eq 1.36E-01 0 9.28E-03 7.16E-04 0 -4.56E-02
Depletion potential of the stratospheric ozone layer (ODP) kg CFC11 eq 7.97E-10 0 1.35E-13 4.96E-11 0 -2.95E-09
Acidification potential of land and water (AP) mol H+ eq 3.57E-01 0 4.6E-03 7.43E-03 0 3.16E-01
Eutrophication potential aquatic freshwater (EP-freshwater) kg P eq 2.19E-03 0 4.92E-06 9.88E-06 0 -5.95E-04
Eutrophication potential aquatic marine (EP-marine) kg N eq 1.43E-01 0 2.11E-03 1.67E-03 0 6.85E-02
Eutrophication potential terrestrial (EP-terrestrial) mol N eq 1.31E+00 0 2.36E-02 1.75E-02 0 8.11E-01
Formation potential of tropospheric ozone photochemical oxidants kg NMVOC
4.83E-01 0 4.13E-03 4.51E-03 0 2.91E-01
(POCP) eq
Abiotic depletion potential for non fossil resources (ADPE) kg Sb eq 1.52E-05 0 1.39E-07 9.23E-07 0 -6.33E-05
Abiotic depletion potential for fossil resources (ADPF) MJ 3.52E+02 0 1.81E+01 6.15E+01 0 -6.59E+03
m3 world eq
Water use (WDP) 1.52E+01 0 1.54E-02 7.72E-01 0 -2.17E+01
deprived
RESULTS OF THE LCA - INDICATORS TO DESCRIBE RESOURCE USE according to EN 15804+A2: 1 m³ sawn timber (459
kg/m³)
Parameter Unit A1-A3 C1 C2 C3 C4 D
Renewable primary energy as energy carrier (PERE) MJ 2.14E+03 0 1.25E+00 7.62E+03 0 -2.03E+03
Renewable primary energy resources as material utilization
MJ 7.59E+03 0 0 -7.59E+03 0 0
(PERM)
Total use of renewable primary energy resources (PERT) MJ 9.73E+03 0 1.25E+00 3.41E+01 0 -2.03E+03
Non renewable primary energy as energy carrier (PENRE) MJ 3.53E+02 0 1.82E+01 6.15E+01 0 -6.59E+03
Non renewable primary energy as material utilization (PENRM) MJ 0 0 0 0 0 0
Total use of non renewable primary energy resources (PENRT) MJ 3.53E+02 0 1.82E+01 6.15E+01 0 -6.59E+03
Use of secondary material (SM) kg 0 0 0 0 0 0
Use of renewable secondary fuels (RSF) MJ 0 0 0 0 0 7.59E+03
Use of non renewable secondary fuels (NRSF) MJ 0 0 0 0 0 0
Use of net fresh water (FW) m3 6.21E-01 0 1.45E-03 3.25E-02 0 -1.38E+00
RESULTS OF THE LCA – WASTE CATEGORIES AND OUTPUT FLOWS according to EN 15804+A2:
1 m³ sawn timber (459 kg/m³)
Parameter Unit A1-A3 C1 C2 C3 C4 D
Hazardous waste disposed (HWD) kg 1.77E-07 0 9.61E-11 5.32E-09 0 -8.17E-07
Non hazardous waste disposed (NHWD) kg 1.86E+00 0 2.96E-03 4.63E-02 0 2.28E-01
Radioactive waste disposed (RWD) kg 5.77E-03 0 3.37E-05 9.82E-03 0 -5.84E-01
Components for re-use (CRU) kg 0 0 0 0 0 0
Materials for recycling (MFR) kg 0 0 0 0 0 0
Materials for energy recovery (MER) kg 0 0 0 4.59E+02 0 0
Exported electrical energy (EEE) MJ 0 0 0 0 0 0
Exported thermal energy (EET) MJ 0 0 0 0 0 0
RESULTS OF THE LCA – additional impact categories according to EN 15804+A2-optional:
1 m³ sawn timber (459 kg/m³)
Parameter Unit A1-A3 C1 C2 C3 C4 D
Disease
Incidence of disease due to PM emissions (PM) ND ND ND ND ND ND
incidence
6 Environmental Product Declaration - Rubner Holding AG - S.p.A - Rubner Sawn Timber, Rubner Sawn Timber kiln dried, Rubner Sawn Timber machine graded
Human exposure efficiency relative to U235 (IR) kBq U235 eq ND ND ND ND ND ND
Comparative toxic unit for ecosystems (ETP-fw) CTUe ND ND ND ND ND ND
Comparative toxic unit for humans (carcinogenic) (HTP-c) CTUh ND ND ND ND ND ND
Comparative toxic unit for humans (noncarcinogenic) (HTP-nc) CTUh ND ND ND ND ND ND
Soil quality index (SQP) SQP ND ND ND ND ND ND
The additional and optional impact categories according to EN 15804+A2 are not declared, as the uncertainty of these indicators is to
be classified as high.
Disclaimer 1 – for the indicator 'Potential Human exposure efficiency relative to U235'.
This impact category deals mainly with the eventual impact of low-dose ionizing radiation on human health of the nuclear fuel cycle. It
does not consider effects due to possible nuclear accidents, occupational exposure or radioactive waste disposal in underground
facilities. Potential ionizing radiation from the soil, radon and from some construction materials is also not measured by this indicator.
Disclaimer 2 – for the indicators 'abiotic depletion potential for non-fossil resources', 'abiotic depletion potential for fossil resources',
'water (user) deprivation potential, deprivation-weighted water consumption', 'potential comparative toxic unit for ecosystems', 'potential
comparative toxic unit for humans – cancerogenic', 'Potential comparative toxic unit for humans - not cancerogenic', 'potential soil
quality index'.
The results of this environmental impact indicator shall be used with care as the uncertainties on these results are high as there is
limited experience with the indicator.
6. LCA: Interpretation
The following interpretation contains a summary of the LCA After its use in the building, the product is assumed to be
results referenced to a declared unit of 1 m³ of sawn timber. incinerated in a biomass power plant. As a result, the
incorporated carbon is emitted again to the atmosphere
The global warming potential (GWP) of sawn timber shows representing biogenic carbon dioxide emissions (module C3).
negative values in the production phase (modules A1–A3). The negative values in the end-of-life (module D) result from
These negative impacts result from the use of wood as raw the energetic treatment of the product. As the energy produced
material. Wood sequesters biogenic carbon during tree growth. at the biomass power plant can substitute (mainly fossil) fuels,
The sequestered carbon does not contribute to global warming an environmental net benefit is generated.
as long as it is stored in the biomass.
In the environmental profile of sawn timber, the upstream steps Due to the use of green electricity in the production, the
for the use of fresh sawn timber represent a driving force in the external supply of electricity at the site represents a minor
contribution to global warming (GWP) as well as in the use of factor in the environmental profile of the product.
fossil resources (ADP fossil). This is primarily due to the
environmental burdens from the forestry processes for The declared results are representative for 100 % of the sawn
roundwood supply. timber produced.
7 Environmental Product Declaration - Rubner Holding AG - S.p.A - Rubner Sawn Timber, Rubner Sawn Timber kiln dried, Rubner Sawn Timber machine graded
7. Requisite evidence
The following evidence of environmental and health relevance 7.4 VOC emissions
was provided. For the verification of VOC emissions, one test report (51005-
002 III B, 2016) of an emission analysis according to AgBB-
7.1 Formaldehyde Scheme 2015 for pure wood is available. Analysis was
Not relevant, as no adhesives containing formaldehyde are performed in accordance with ISO 16000-3 and ISO 16000-6.
used in the production process. A test report (No. The listed values represent lower limit values.
2117078/CT/2022/1/A1, 2022) confirms a formaldehyde
emission below the technical detection limit.
VOC emissions
Name Value Unit
7.2 MDI
Not relevant, as no MDI-containing adhesives are used in the TVOC (C6 - C16) acc. to AgBB 2015 10 μg/m3
production process. Sum SVOC (C16 - C22) acc. to AgBB 2015 < 5 μg/m3
R (dimensionless) acc. to AgBB 2015 0.086 -
7.3 Fire gas toxicity
VOC without NIK acc. to AgBB 2015 < 5 μg/m3
The toxicity of the fire gases produced by the fire corresponds
to the toxicity of the fire gases produced by the fire of natural
wood.
8. References
Standards Part 2: Estimation by electrical resistance method.
DIN 53436 EN 13501-1
DIN 53436:2015, Generation of thermal decomposition ÖNORM EN 13501-1, Fire classification of construction
products from materials for their analytic-toxicological testing. products and building elements -
Part 1: Classification using data from reaction to fire tests.
DIN 68800-2
DIN 68800-2:2012-02, Wood preservation – Part 2: Preventive EN 15804
constructional measures in buildings. DIN EN 15804:2012+A2:2019+AC:2021, Sustainability of
construction works Environmental product declarations Core
DIN 68800-3 rules for the product category of construction products.
DIN 68800-3:2012-02, Wood preservation – Part 3: Preventive
protection of wood with wood preservatives. hEN 14081
hEN 14081-1:2016-06-01, Timber structures - Strength graded
EN 336 structural timber with rectangular cross section - Part 1:
EN 336:2013-12, Structural timber - Sizes, permitted General requirements.
deviations.
ISO 12572
EN 338 EN ISO 12572:2016, Hygrothermal performance of building
DIN EN 338:2016-07, Structural timber - Strength classes. materials and products - Determination of water vapour
transmission properties - Cup method.
EN 717-1
DIN EN 717-1:2005-01, Wood-based panels – Determination of ISO 14025
Formaldehyde release – Part 1: Formaldehyde emission by the DIN EN ISO 14025:2011-10, Environmental labels and
chamber method. declarations Type III environmental declarations Principles and
procedures.
EN 1912
EN 1912:2013-10-15, Structural timber - Strength classes - ISO 14044
Assignment of visual grades and species. DIN EN ISO 14044:2006-10, Environmental management - Life
cycle assessment - Requirements and guidelines.
EN 1995-1-1
OEN 1995-1-1, Eurocode, 5: Bemessung und Konstruktion von ISO 16000-3
Holzbauten - Teil 1-1: Allgemeines - Allgemeine Regeln und ISO 16000-3:2011, Indoor air - Part 3: Determination of
Regeln für den Hochbau - Konsolidierte Version mit nationalen formaldehyde and other carbonyl compounds in indoor air and
Festlegungen, nationalen Erläuterungen und nationalen test chamber air - Active sampling method.
Ergänzungen zur Umsetzung der ÖNORM EN 1995-1-1,
german Version ISO 16000-6
ISO 16000-6:2011, Indoor air - Part 6: Determination of volatile
EN 12664 organic compounds in
EN 12664:2001, Thermal performance of building materials and indoor and test chamber air by active sampling on Tenax TA®
products - Determination of thermal resistance by means of sorbent, thermal desorption and gas chromatography using MS
guarded hot plate and heat flow meter methods - Dry and moist or MS-FID.
products with medium and low thermal resistance.
EN 13183-2
EN 13183-2:2002, Moisture content of a piece of sawn timber -
8 Environmental Product Declaration - Rubner Holding AG - S.p.A - Rubner Sawn Timber, Rubner Sawn Timber kiln dried, Rubner Sawn Timber machine graded
Further references Assessment and Requirements on the Project Report according
to EN 15804+A2:2019. Version 1.3. Berlin: Institut Bauen und
AgBB-Scheme 2015 Umwelt e.V., 2022.
German Committee for HealthRelated Evaluation of Building
Products (AgBB): Approach to health assessment of emissions PCR: Solid wood products
of volatile organic compounds (VOCs and SVOCs) from Product category rules for building-related products and
building products. services. Part B: EPD requirements for solid wood products.
Version v2, Berlin: Institut Bauen und Umwelt e.V., 31.05.2023.
Candidate List
List of substances of very high concern considered for approval PCR 305/2011 (EU)
(status 17.01.2023) according to Article 59 para. 10 of the REGULATION (EU) No 305/2011 OF THE EUROPEAN
REACH Regulation. European Chemicals Agency. PARLIAMENT AND OF THE COUNCIL of 9 March 2011 laying
down harmonised conditions for the marketing of construction
GaBi products and repealing Council Directive 89/106/EEC.
GaBi 10, Software-System and Database for Life Cycle
Engineering. 2022.2. Stuttgart, Echterdingen: Sphera, 1992- Rüter & Diederichs 2012
2022. Available at: https://sphera.com/product-sustainability- Ökobilanz-Basisdaten für Bauprodukte aus Holz. Work report
gabi-data-search/ from the Institut für Holztechnologie und Holzbiologie Nr.
2012/1. Hamburg: Johann Heinrich von Thünen-Institut.
IBU 2021
Institut Bauen und Umwelt e.V.: General Programme 1907/2006/EG
Instructions for the Preparation of EPDs at the Institut Bauen VERORDNUNG (EG) Nr. 1907/2006 DES EUROPÄISCHEN
und Umwelt e.V. (IBU). Version 2.0, Berlin: Institut Bauen und PARLAMENTS UND DES RATES vom 18. Dezember 2006 zur
Umwelt e.V., 2021. www.ibuepd.com Registrierung, Bewertung, Zulassung undBeschränkung
chemischer Stoffe (REACH).
Meyer, 1994
Meyer, B, Boehme, C: 1994, Formaldeyhdabgabe von natürlich 2014/955/EU
gewachsenem Holz, Holzzentralblatt 122 (Formaldeyhd release 2014/955/EU,COMMISSION DECISION of 18 December 2014
of naturally grown wood), S 1969-1972. amending Decision 2000/532/EC on the list of waste pursuant
to Directive 2008/98/EC of the European Parliament and of the
PCR part A Council.
Product category rules for building-related products and
services. Part A: Calculation Rules for the Life Cycle
9 Environmental Product Declaration - Rubner Holding AG - S.p.A - Rubner Sawn Timber, Rubner Sawn Timber kiln dried, Rubner Sawn Timber machine graded
Publisher
Institut Bauen und Umwelt e.V. +49 (0)30 3087748- 0
Hegelplatz 1 info@ibu-epd.com
10117 Berlin www.ibu-epd.com
Germany
Programme holder
Institut Bauen und Umwelt e.V. +49 (0)30 3087748- 0
Hegelplatz 1 info@ibu-epd.com
10117 Berlin www.ibu-epd.com
Germany
Author of the Life Cycle Assessment
Daxner & Merl GmbH +43 676 849477826
Schleifmühlgasse 13/24 office@daxner-merl.com
1040 Wien www.daxner-merl.com
Austria
Owner of the Declaration
Rubner Holding AG - S.p.A. 0039 0474 563 777
Handwerkerzone 2 info@rubner.com
39030 Kiens www.rubner.com
Italy
10 Environmental Product Declaration - Rubner Holding AG - S.p.A - Rubner Sawn Timber, Rubner Sawn Timber kiln dried, Rubner Sawn Timber machine graded
