ENVIRONMENTAL PRODUCT DECLARATION
as per ISO 14025 and EN 15804+A2
Owner of the Declaration Hansgrohe Group
Publisher Institut Bauen und Umwelt e.V. (IBU)
Programme holder Institut Bauen und Umwelt e.V. (IBU)
Declaration number EPD-HAN-20240196-ICC1-EN
Issue date 03.12.2024
Valid to 02.12.2029
Shower Sets - EcoSmart
Hansgrohe Group
www.ibu-epd.com | https://epd-online.com
1. General Information
Hansgrohe Group Shower Sets - EcoSmart
Programme holder Owner of the declaration
IBU – Institut Bauen und Umwelt e.V. Hansgrohe Group
Hegelplatz 1 Auestr. 5-9
10117 Berlin 77761 Schiltach
Germany Germany
Declaration number Declared product / declared unit
EPD-HAN-20240196-ICC1-EN one piece of an average shower set EcoSmart
This declaration is based on the product category rules: Scope:
Fittings and showers, 01.08.2021 This average EPD covers the most relevant chrome plated shower sets
(PCR checked and approved by the SVR) equipped with EcoSmart technology based on criteria like sales volume,
long-term relevance and price point.
The owner of the declaration shall be liable for the underlying information
Issue date and evidence; the IBU shall not be liable with respect to manufacturer
information, life cycle assessment data and evidences.
03.12.2024
The EPD was created according to the specifications of EN 15804+A2. In
the following, the standard will be simplified as EN 15804.
Valid to
02.12.2029 Verification
The standard EN 15804 serves as the core PCR
Independent verification of the declaration and data according to ISO
14025:2011
internally X externally
Dipl.-Ing. Hans Peters
(Chairman of Institut Bauen und Umwelt e.V.)
Florian Pronold Dr Naeem Adibi,
(Managing Director Institut Bauen und Umwelt e.V.) (Independent verifier)
1 Environmental Product Declaration - Hansgrohe Group - Shower Sets - EcoSmart
2. Product
The material composition (incl. packaging) of an average
2.1 Product description/Product definition EcoSmart shower set is as follows:
Shower sets essentially comprise of hand shower, shower hose
plus shower bar.
Name Value Unit
Brass 24.8 %
A hand shower consists of a housing made of plastic materials
or metal and a jet disc as well as several assembly parts of Plastic 22.7 %
various materials. A shower hose is a plastic hose with metal Cardboard, Paper 19.2 %
connectors, made of brass or stainless steel. The shower bar PVC 13.7 %
surface is usually chrome-plated by means of various galvanic
ABS 10.1 %
process stages.
Zinc 5.4 %
The EcoSmart technology reduces the water consumption of Coating metals 1.7 %
the products which ensures efficient use of water. Stainless Steel 1.4 %
Steel 0.5 %
For the use and application of the product the respective
Aluminium 0.3 %
national provisions at the place of use apply, in Germany for
Other material 0.3 %
example the building codes of the federal states and the
corresponding national specifications.
The products comply with the applicable standards and The parts which are made of brass contain between 0.2 and
regulations listed below. 1.4% lead.
This product contains substances listed in the candidate list
Following standards apply to all shower sets to prove product (date: 17.12.2021) exceeding 0.1 percentage by mass: Lead
safety: (CAS number 7439-92-1) as a component of the brass alloy
has been on the candidate list of the Reach Regulation
• EN 1112:2008: Sanitary tapware – Shower outlets for
(Regulation (EC) No. 1907/2006) since 27.06.2018.
sanitary tapware for water supply systems of type 1 and
type 2
This product/article/at least one partial article contains other
• EN 1113:2015: Sanitary tapware – Shower hoses for
CMR substances in categories 1A or 1B which are not on the
sanitary tapware for water supply systems of type 1 and
candidate list, exceeding 0.1 percentage by mass: no.
type 2
• ISO 3822: Acoustics – Laboratory tests on noise
Biocide products were added to this construction product or it
emission from appliances and equipment used in water
has been treated with biocide products (this then concerns a
supply installations
treated product as defined by the (EU) Ordinance on Biocide
2.2 Application Products No. 528/2012): no.
Shower sets are a combination of a hand shower, a shower
2.6 Manufacture
hose and a shower bar. The shower bar enables the shower
Hand shower:
head to be fixed at any height. They are used in bathrooms for
showering or in bathtubs.
2.3 Technical Data
Constructional data
Name Value Unit
Maximum load temperature
42 °C
permanent operation
Maximum load temperature
70 °C
temporary operation
Flow rate (indications for Depending on flow rate
m3/h
pressure range of 1-3 bar) class 0,396 to 0,57
Sound emissions <30 dB
Performance data of the product with respect to its
characteristics in accordance with the relevant technical
provision (no CE-marking).
2.4 Delivery status
The shower sets are delivered singularly packaged. The
packaging is customized to the size of the product and
supplies. Customers can order single products or multiple
No. 1: The plastic handle of the hand showers is injected.
products with outer packaging. The products with the smallest
No. 2: The handle is galvanized with chrome.
and the largest volume have dimensions between 730x152x65
No. 3: The plastic inlet housing is injected.
mm and 990x165x75 mm.
No. 4: The plastic pipe bow is injected.
No. 5: The plastic distributor is injected.
2.5 Base materials/Ancillary materials
No. 6: Meanwhile, the plastic jet body is injected.
2 Environmental Product Declaration - Hansgrohe Group - Shower Sets - EcoSmart
No. 7: The distributor and the jet body are preassembled.
No. 8: All the parts are assembled and packed. 2.9 Packaging
For product protection the shower sets are individually packed
Shower hose: in a cardboard box, which consists of approximately 80%
recycled material. The cardboard is always printed with lead-
free ink and clear dispersion varnish. The inlay of the packaging
consists of folded cardboard, fiber form or plastic bags,
depending on the product. The packaging can be fully recycled.
2.10 Condition of use
To protect the shower sets and make them durable, the product
is usually chrome-plated. Nevertheless, it will not release
unhealthy contaminants in the water, if used as intended. To
ensure the longevity of the product, it should be used and
cleaned regularly.
2.11 Environment and health during use
Our products do not emission any contaminants or substances
that are harmful to the environment or health during the use
phase.
2.12 Reference service life
The quality and durability of our shower sets is designed for a
product life of about 20 years. Which on average is
approximately the duration of use by the consumers.
Nevertheless, it is possible that some parts are needed to be
No. 1: The TPE inner tube is extruded.
changed earlier (like shower hoses).
No. 2: The PVC top layer is applied on the inner tube.
No. 3: The embossing foil chrome is applied on the top layer.
With few exceptions, all products have a five-year warranty.
No. 4: The hose is cut in length and assembled with the
Furthermore, an after-sale service warranty of 15 years is
connections.
provided.
Packaging:
In the end all components are packed together with some 2.13 Extraordinary effects
additional parts like shower bar and slider. Fire
The products are not classified as building materials (building
Any production waste generated is disposed accordingly. In products) and are not subject to DIN 4102 and EN 13501-1.
individual cases, the production may differ slightly from the
Fire protection
procedure
Name Value
2.7 Environment and health during manufacturing Building material class -
Hansgrohe SE tries to keep the impact on people and the
Burning droplets -
environment as low as possible when manufacturing its
Smoke gas development -
products.
Hazards at workplaces are regularly assessed and reduced to a
minimum. Water
For example, in basic production, sawing or grinding work is If a room in which the products offered by Hansgrohe are
mainly carried out by robots, and in electroplating, chemicals installed is flooded with water, the products are not affected in
are dosed automatically via appropriate pump stations. their function. There will be no environmental impact.
Emissions that are hazardous to health are extracted directly at
the source and cleaned by filter systems. Mechanical destruction
Workplace and emission limits are regularly monitored and are If the surface of the coating is destroyed by a mechanical
far below the prescribed limits. stress, there is a possibility of corrosion. In the event of
To reduce environmental impact, water and production waste mechanical damage, the products may need to be replaced
are recycled wherever possible. due to possible sharp cut edges.
In addition, all production sites are certified according to the
2.14 Re-use phase
DIN EN ISO standards 14001 (environment), 50001 (energy),
45001 (occupational health and safety) and 9001 (quality). The shower sets are not taken back by the manufacturer for the
Continuous improvement of environmental and occupational purpose of reuse. Users can disassemble the products
safety performance is thus guaranteed. repeatedly within the reference utilization period and reuse it
elsewhere.
2.8 Product processing/Installation
2.15 Disposal
Make holes in the wall for the fixation of the shower bar (tool:
drilling machine) and insert dowels and silicone (tool: silicon The waste code of the product is AVV 20 03 01. Disassembly of
injector). the products consists of the same steps as assembly, in
Screw on the shower bar (tool: screwdriver) and attach the reverse order. All metal components can be recycled (as
cover caps. scrap).All plastic components have a high calorific value and
Screw the shower hose with union nut and seal onto the wall can be sent for thermal recycling. In countries where no thermal
outlet by hand. recycling or substance recycling is established, disposal takes
Screw the shower hose with union nut and seal onto the hand place via the waste incineration plant.
shower by hand.
3 Environmental Product Declaration - Hansgrohe Group - Shower Sets - EcoSmart
https://www.hansgrohe.com.
2.16 Further information
Additional information about our products can be found at
3. LCA: Calculation rules
Module D:
3.1 Declared Unit Identification of the benefits and costs of the product outside
The results of this EPD are valid for the following functional the system boundary. For waste, paper and plastics, these
unit: consist of energy credits from thermal utilization (A3, A5 and
Provide sanitary function for one (1) average shower set unit C3) in the form of the average European electricity mix or
used in accordance with the manufacturer's recommendations thermal energy from natural
for a 20-year life, following the manufacturer's operating gas. Recycling of paper, plastic and metal scrap results in
instructions. An average conditioned shower set is considered credits of the respective raw materials for the primary material
the baseline flow. portion of the input. The loads of the waste incineration and
recycling processes are assigned to the respective modules
Weighted averaging based on production tonnages in 2022/23 (A3, A5 and C3) and not to module D.
is chosen as basis for creating the environmental profile. 14
different shower sets were considered. 3.3 Estimates and assumptions
Energy and water consumption, material amount for coating as
Declared unit
well as waste during production could only be determined on
Name Value Unit
concrete, existing products and not on the average product.
Declared unit 1 pce. The highest value of all inputs and outputs for energy, waste
Declared unit with packaging 1.272 kg and coating of the top seller, the lightest and the heaviest
Packaging 0.264 kg product was used for the calculation of energy, water, waste
and coating.
Weight range of the products 1.069-1.972 kg
For the incineration with energy recovery (thermal and electric)
Mass reference 1.272 kg/pce
of waste, an r1 value of > 0.6 is assumed. The net efficiency for
the average waste incinerated is between 38 % and 44 %,
depending on the type of waste respectively the disposal data
3.2 System boundary set.
This representative EPD follows the EPD type "cradle to gate -
with options". The following life cycle modules are declared: 3.4 Cut-off criteria
Modules A1-A3: The effect associated with the neglected mass shares is less
The product stage begins with considering the production of the than 5% of the effect categories per module. The minimum limit
necessary raw materials and of 1% total mass and the use of renewable and nonrenewable
energies, including all corresponding upstream chains and the primary energy is not exceeded.
actual procurement transports. Furthermore, the entire
3.5 Background data
manufacturing phase was mapped, including the treatment of
production waste until the end-of- waste status (EoW) was The LCA software LCA for Experts (GaBi) 10.7 was used to
reached. Green electricity from hydropower is used for the model the life cycle. The entire manufacturing process, as well
manufacturing processes in Germany. Green electricity from as energy consumption, were modelled on the basis of
hydropower and wind power (50% each) is used for the French manufacturer specific data.
production site. US electricity mix is used for the US production However, generic background datasets were used for the
site. upstream and downstream processes. The majority of the
Module A4: background datasets used were taken from the current version
All distribution transports to the customers were considered. (2023.2) of the GaBi database. Ecoinvent Version 3.9 (2021)
Module A5: datasets were only used when suitable GaBi datasets were not
This module covers the installation process with the available.
corresponding packaging waste generated that needs to be
3.6 Data quality
disposed.
The background datasets used for accounting purposes mainly
Modules B1 & B3-B5:
originate from the respective updated GaBi databases at the
These modules were considered, but evaluated as not relevant
time of calculation. The data for the examined products was
for the products and considered as zero.
captured on the basis of evaluations of internal production and
Module B2:
environmental data, the collection of LCA relevant data within
Maintenance expenses are declared in this module and consist
the supply chain, as well as the evaluation of relevant data for
of weekly cleaning expenses for this product.
the energy supply. The collected data were checked for
Module B6:
plausibility and consistency.
This module considers the energy input required to bring water
Good representativity can be assumed.
to a certain temperature for the use of a gas low temperature
For the assessment of the variability of the results, all products
boiler (scenario B6/1) and for the use of an electric
were balanced in addition to the average product. See at
instantaneous water heater (scenario B6/2).
chapter 6 for explanation of the variability.
Module B7:
This module considers the water consumption that can be
3.7 Period under review
expected depending on the function of the product family.
Life cycle assessment data were collected in 2022/23.
Modules C1-C4:
The modules include the environmental impacts for dismantling 3.8 Geographic Representativeness
of the products and the treatment of the waste fractions until
Land or region, in which the declared product system is
the end-of-waste status (EoW) is reached, including the
manufactured, used or handled at the end of the product´s
associated transports at the end of the product life cycle.
lifespan: Europe
4 Environmental Product Declaration - Hansgrohe Group - Shower Sets - EcoSmart
Packaging:
3.9 Allocation For paper and cardboard, recycling (91 %) and energy recovery
For the production process nearly all raw materials, precursors (9 %) are considered on a pro rata basis. For plastic, a
and supplies could be assigned to the declared product. proportionate recycling (52 %), energy recovery (48 %)
Energy, water, galvanization process and production waste considered, based on Eurostat.
were assigned to the highest value of either the heaviest, Deconstructed product at the end of life:
lightest or most sold product of the product group. No Since the product has a high plastic content, it is assumed that
byproducts are produced and no allocation is required. 95% of the plastic and metal components are incinerated (C3)
Some of the brass losses from brass processing in module A3 and 5% are disposed in landfill (C4). The metal components are
are directly reused by Hansgrohe and are modelled as a closed incinerated without energy recovery and the plastic
loop. Another part of the brass losses (brass particles and components are incinerated with energy recovery.
dusts) is disposed of as waste (without debits and credits).
Credits for plastics, paper and cardboard recycled in A5 and 3.10 Comparability
metallurgical waste in C3 are credited in module D. Basically, a comparison or an evaluation of EPD data is only
Credits for the energy recovery of incinerated production waste possible if all the data sets to be compared were created
in A1-3, paper, cardboard and plastics in A5 and plastics and according to EN 15804 and the building context, respectively
other materials in C3 are credited in module D. the product-specific characteristics of performance, are taken
The loads for waste water treatment and waste disposal of core into account. The background database used is LCA for
sand, waste oil and hazardous waste from the manufacturing Experts (GaBi) 10.7 in the
phase are allocated to module A3. database version 2023.2.
4. LCA: Scenarios and additional technical information
Characteristic product properties of biogenic carbon
Service life
The biogenic carbon content was calculated based on the
Hansgrohe SE declares a Service Life of 20 years as an
factors from the Thünen Intitute.
empirical value for the shower sets EcoSmart when used in
Information on describing the biogenic carbon content at accordance with the care instructions. This value is based on
factory gate their technical service centre's statistics on service life in the
Name ValueUnit market and complaints.
kg Name Value Unit
Biogenic carbon content in product -
C Life Span according to the manufacturer 20 a
Biogenic carbon content in accompanying kg
0.1
packaging C Operational energy use (B6) and Operational water use
(B7)
Note: 1 kg of biogenic carbon is equivalent to 44/12 kg of CO .
2 Modules B6 and B7 are calculated based on the directions of
the IBU PCR part B.
Module B6 considers the operational energy use. Scenario B6
The following technical information is a basis for the declared
assumes the use of a gas low temperature boiler. Scenario
modules.
B6/1 assumes the use of an electric instantaneous water heater
(21 kW). Module B7 considers the operational water use.
Transport to the building site (A4)
Name Value Unit
Name ValueUnit Water consumption 61.2 m3
Transport distance 679 km
Energy demand 2846 kWh
Capacity utilisation (including empty runs) (Truck) 55 %
Transport distance (Container ship) 1460 km End of life (C1-C4)
Capacity utilisation (Container ship) 80 % Name Value Unit
Collected separately waste type 1.028 kg
Installation into the building (A5)
Energy recovery 0.978 kg
The packaging is disposed either by recycling or incineration.
Landfilling 0.05 kg
Name Value Unit
Auxiliary (Silicone) 0.02 kg
Reuse, recovery and/or recycling potentials (D), relevant
Electricity consumption 0.002 kWh
scenario information
Packaging (Paper, cardboard, plastic) 0.264 kg The energy generated from energy recovery as well as recycled
materials are assigned to module D as possible potentials or
Maintenance (B2)
avoided loads in subsequent systems. Credits are only given
For module B2, it is assumed that a weekly cleaning of the for the primary portion of the inputs.
product takes place, with 0.5 liter of water containing 1.5%
soap.
Name Value Unit
Maintenance cycle (cleaning) 780 Number/RSL
Water consumption/Cycle weekly
0.5 Liter/cycle
(cleaning)
Soap concentration (cleaning) 1.5 %
Water consumption (cleaning) 0.52 m3
Auxiliary Soap/Tensides (cleaning) 7.8 kg
5 Environmental Product Declaration - Hansgrohe Group - Shower Sets - EcoSmart
5. LCA: Results
The following table shows the result of the LCA for 1 piece of an average shower set EcoSmart. The results in the B-module are based
on a lifetime of 20 years. Scenario B6 shows the result for the use of a gas low temperature boiler. Scenario B6/1 shows the result for
the use of an electric instantaneous water heater.
DESCRIPTION OF THE SYSTEM BOUNDARY (X = INCLUDED IN LCA; MND = MODULE OR INDICATOR NOT DECLARED; MNR
= MODULE NOT RELEVANT)
Benefits and
Construction loads beyond
Product stage Use stage End of life stage
process stage the system
boundaries
la ire ta m w a Ry lp p u s tro p s n a rT g n iru tc a fu n a M e h t m o rf tro p s n a rTe tis e h t o t e ta g y lb m e s s A e s U e c n a n e tn ia M ria p e R tn e m e c a lp e R tn e m h s ib ru fe R y g re n e la n o ita re p Oe s u re ta w la n o ita re p Oe s u n o itc u rts n o c -e Dn o itilo m e d tro p s n a rT g n is s e c o rp e ts a W la s o p s iD -e s u e R-y re v o c e R-g n ilc y c e Rla itn e to p
A1 A2 A3 A4 A5 B1 B2 B3 B4 B5 B6 B7 C1 C2 C3 C4 D
X X X X X X X X X X X X X X X X X
RESULTS OF THE LCA - ENVIRONMENTAL IMPACT according to EN 15804+A2: 1 piece average shower set EcoSmart
Parameter Unit A1-A3 A4 A5 B1 B2 B3 B4 B5 B6 B6/1 B7 C1 C2 C3 C4 D
GWP-total kg CO 2 3.74E 1.02E- 5.44E- 0 2.42E 0 0 0 7.57E 9.18E 3.29E 0 1.96E- 1.32E 2.98E-03 -9.51E-
eq +00 01 01 +01 +02 +02 +01 02 +00 01
GWP-fossil kg CO 2 4.1E+00 1.02E- 1.77E- 0 1.82E 0 0 0 7.56E 9.18E 3.28E 0 1.94E- 1.32E 2.98E-03 -5.9E-01
eq 01 01 +01 +02 +02 +01 02 +00
GWP- kg CO 2 -3.66E- 0 3.66E- 0 0 0 0 0 0 0 0 0 0 0 0 -3.62E-
biogenic eq 01 01 01
GWP-luluc kg CO 2 4.94E-03 7.56E- 1.84E- 0 6.02E 0 0 0 2.59E- 9.98E- 9.37E- 0 1.79E- 1.06E- 2.7E-06 3.82E-05
eq 04 04 +00 02 02 03 04 04
kg CFC11 1.09E- 1.67E- 1.69E- 2.17E- 2.52E- 1.79E- -8.16E-
ODP 3.04E-09 1.2E-14 8.11E-13 0 0 0 0 0 4.99E-15
eq 06 10 08 10 15 10 10
8.02E- 4.74E- 6.64E- 4.59E- 1.96E 8.17E- 3.14E- 5.79E-
AP mol H+ eq 3.22E-02 0 0 0 0 0 9.25E-06 2.32E-05
04 04 02 01 +00 02 05 04
EP- 3.03E- 3.17E- 5.81E- 7.62E- 3.42E- 3.86E- 7.07E- 2.22E- -3.58E-
kg P eq 2.24E-05 0 0 0 0 0 3.77E-07
freshwater 07 07 04 05 03 02 08 07 06
2.15E- 1.08E- 1.51E- 1.99E- 4.69E- 1.67E- 1.22E- 2.47E- -2.04E-
EP-marine kg N eq 2.67E-03 0 0 0 0 0 2.22E-06
04 04 02 01 01 01 05 04 04
2.39E- 1.18E- 1.81E- 2.17E 2.44E- 2.92E- -2.15E-
EP-terrestrial mol N eq 2.78E-02 0 0 0 0 4.9E+00 0 1.4E-04 2.42E-05
03 03 01 +00 01 03 03
kg
5.84E- 3.66E- 6.03E- 5.77E- 1.25E 6.17E- 6.51E- -4.94E-
POCP NMVOC 9.35E-03 0 0 0 0 0 2.8E-05 6.99E-06
04 04 02 01 +00 02 04 04
eq
5.59E- 2.69E- 9.18E- 1.42E- 1.54E- 1.28E- 3.28E-
ADPE kg Sb eq 5.15E-04 0 2.1E-05 0 0 0 0 8.02E-11 3.57E-05
09 06 06 04 06 09 09
1.35E 2.48E 4.52E 1.28E 1.93E 3.67E 2.64E- 1.33E -9.97E
ADPF MJ 7.9E+01 0 0 0 0 0 4.44E-02
+00 +00 +02 +04 +04 +02 01 +00 +00
m3 world
1.02E- 5.41E- 6.94E 2.47E 2.05E 1.14E 2.34E- -3.83E- -5.49E-
WDP eq 1.57E-01 0 0 0 0 0 1.3E-01
03 02 +00 +00 +02 +01 04 05 03
deprived
GWP = Global warming potential; ODP = Depletion potential of the stratospheric ozone layer; AP = Acidification potential of land and water; EP =
Eutrophication potential; POCP = Formation potential of tropospheric ozone photochemical oxidants; ADPE = Abiotic depletion potential for non-fossil
resources; ADPF = Abiotic depletion potential for fossil resources; WDP = Water (user) deprivation potential)
RESULTS OF THE LCA - INDICATORS TO DESCRIBE RESOURCE USE according to EN 15804+A2: 1 piece average shower set
EcoSmart
Parameter Unit A1-A3 A4 A5 B1 B2 B3 B4 B5 B6 B6/1 B7 C1 C2 C3 C4 D
1.81E 9.38E 1.26E 1.15E 1.38E -4.44E
PERE MJ 8.2E-02 5.28E+00 0 0 0 0 0 1.92E-024.22E-01 4.03E-03
+01 +01 +02 +04 +02 +00
4.05E -4.05E
PERM MJ 0 0 0 0 0 0 0 0 0 0 0 0 0 0
+00 +00
2.22E 9.38E 1.26E 1.15E 1.38E -4.44E
PERT MJ 8.2E-02 1.23E+00 0 0 0 0 0 1.92E-024.22E-01 4.03E-03
+01 +01 +02 +04 +02 +00
6.08E 1.36E 4.52E 1.28E 1.93E 3.67E 1.82E -9.97E
PENRE MJ 3.09E+00 0 0 0 0 0 2.65E-01 9.31E-01
+01 +00 +02 +04 +04 +02 +01 +00
1.83E -6.02E- -1.69E -8.87E-
PENRM MJ 0 0 0 0 0 0 0 0 0 0 0 0
+01 01 +01 01
7.92E 1.36E 4.52E 1.28E 1.93E 3.67E 1.33E -9.97E
PENRT MJ 2.49E+00 0 0 0 0 0 2.65E-01 4.45E-02
+01 +00 +02 +04 +04 +02 +00 +00
SM kg 5.22E-01 0 0 0 0 0 0 0 0 0 0 0 0 0 0 4.01E-02
RSF MJ 1.52E-23 0 0 0 0 0 0 0 0 0 0 0 0 0 0 0
NRSF MJ 1.78E-22 0 0 0 0 0 0 0 0 0 0 0 0 0 0 0
6 Environmental Product Declaration - Hansgrohe Group - Shower Sets - EcoSmart
9.32E
FW m3 2.26E-02 9E-05 1.8E-03 0 1.62E-01 0 0 0 1.22E-01 3.22E-01 0 2.1E-05 3.21E-03 5.42E-07 -1.5E-03
+00
PERE = Use of renewable primary energy excluding renewable primary energy resources used as raw materials; PERM = Use of renewable primary
energy resources used as raw materials; PERT = Total use of renewable primary energy resources; PENRE = Use of non-renewable primary energy
excluding non-renewable primary energy resources used as raw materials; PENRM = Use of non-renewable primary energy resources used as raw
materials; PENRT = Total use of non-renewable primary energy resources; SM = Use of secondary material; RSF = Use of renewable secondary fuels;
NRSF = Use of non-renewable secondary fuels; FW = Use of net fresh water
RESULTS OF THE LCA – WASTE CATEGORIES AND OUTPUT FLOWS according to EN 15804+A2:
1 piece average shower set EcoSmart
Parameter Unit A1-A3 A4 A5 B1 B2 B3 B4 B5 B6 B6/1 B7 C1 C2 C3 C4 D
-1.51E- -8.48E-
HWD kg 3.26E-064.22E-128.05E-11 0 8.5E-03 0 0 0 2.22E-06 0 8.19E-13 1.2E-10 3.7E-12 2.08E-07
06 09
1.99E 1.42E 5.97E
NHWD kg 4.09E-011.92E-043.42E-02 0 6.59E-01 0 0 0 0 4.03E-055.47E-025.13E-021.96E-02
+00 +01 +01
3.07E -4.71E-
RWD kg 1.72E-032.37E-061.27E-04 0 4.14E-03 0 0 0 2.94E-02 3.16E-02 0 4.95E-07 5.6E-05 5.23E-07
+00 04
CRU kg 0 0 0 0 0 0 0 0 0 0 0 0 0 0 0 0
MFR kg 0 0 2.31E-01 0 0 0 0 0 0 0 0 0 0 0 0 0
MER kg 0 0 0 0 0 0 0 0 0 0 0 0 0 0 0 0
2.36E
EEE MJ 1.9E-01 0 1.09E-01 0 0 0 0 0 0 0 0 0 0 4.5E-05 0
+00
4.26E
EET MJ 3.75E-01 0 1.96E-01 0 0 0 0 0 0 0 0 0 0 0 0
+00
HWD = Hazardous waste disposed; NHWD = Non-hazardous waste disposed; RWD = Radioactive waste disposed; CRU = Components for re-use;
MFR = Materials for recycling; MER = Materials for energy recovery; EEE = Exported electrical energy; EET = Exported thermal energy
RESULTS OF THE LCA – additional impact categories according to EN 15804+A2-optional:
1 piece average shower set EcoSmart
Parameter Unit A1-A3 A4 A5 B1 B2 B3 B4 B5 B6 B6/1 B7 C1 C2 C3 C4 D
Disease
PM ND ND ND ND ND ND ND ND 2.94E-06 1.65E-05 ND ND ND ND ND ND
incidence
kBq U235
IR ND ND ND ND ND ND ND ND 4.77E+00 5.11E+02 ND ND ND ND ND ND
eq
ETP-fw CTUe ND ND ND ND ND ND ND ND 1.57E+025.37E+03 ND ND ND ND ND ND
HTP-c CTUh ND ND ND ND ND ND ND ND 4.12E-08 2.84E-07 ND ND ND ND ND ND
HTP-nc CTUh ND ND ND ND ND ND ND ND 4E-06 4.53E-06 ND ND ND ND ND ND
SQP SQP ND ND ND ND ND ND ND ND 8.98E+017.58E+03 ND ND ND ND ND ND
PM = Potential incidence of disease due to PM emissions; IR = Potential Human exposure efficiency relative to U235; ETP-fw = Potential comparative
Toxic Unit for ecosystems; HTP-c = Potential comparative Toxic Unit for humans (cancerogenic); HTP-nc = Potential comparative Toxic Unit for humans
(not cancerogenic); SQP = Potential soil quality index
Disclaimer 1 – for the indicator 'Potential Human exposure efficiency relative to U235'. This impact category deals mainly with the
eventual impact of low-dose ionizing radiation on human health of the nuclear fuel cycle. It does not consider effects due to possible
nuclear accidents, occupational exposure or radioactive waste disposal in underground facilities. Potential ionizing radiation from the
soil, radon and from some construction materials is also not measured by this indicator.
Disclaimer 2 – for the indicators 'abiotic depletion potential for non-fossil resources', 'abiotic depletion potential for fossil resources',
'water (user) deprivation potential, deprivation-weighted water consumption', 'potential comparative toxic unit for ecosystems', 'potential
comparative toxic unit for humans – cancerogenic', 'Potential comparative toxic unit for humans - not cancerogenic', 'potential soil
quality index'. The results of this environmental impact indicator shall be used with care as the uncertainties on these results are high
as there is limited experience with the indicator.
6. LCA: Interpretation
7 Environmental Product Declaration - Hansgrohe Group - Shower Sets - EcoSmart
compared to the average product weighted by production
The dominance analysis shows that modules B2, B6 and B7 volume.
are the dominant life cycle stages in most of the categories. The different types of products all have the same function and
The contribution of B2 is due to the demand of soap and water differ mainly in terms of design, which has an influence on
for cleaning. Module B6 dominates most of the indicators due construction and materials used. The basic structure of the
to the energy demand for water heating and module B7 has a product types is always similar. Material type and quantity
high contribution to EP-freshwater due to the wastewater proportions do not differ much, as also shown in the average
treatment. The module A1-A3 has a very low contribution to all material composition table.
categories except of ADPE. In this indicator the provision of The deviation of the GWP fossil in modules A1-C4 has a
zinc has the largest contribution. The end-of-life stage has no maximum of 9% and a minimum of -23% with a mix scenario of
significant influence on the environmental indicators. 50% B6/1 and 50% B6/2. The deviation of the PENRT in
The environmental burdens from the transports (modules A4 modules A1-C4 has a maximum of 10% and a minimum of -
and C2) account for less than 0.1% of the total burdens of the 23%. The deviation of the NHWD in modules A1-C4 has a
respective indicators in all cases. maximum of 10% and a minimum of -23%. Modules B6 and B7
The possible potentials of avoided loads of subsequent account for more than 90% of the GWP indicator. The deviation
systems (module D) lie outside the considered system from the average is mainly caused by the flow rate in module
boundaries and relate exclusively to credits from recycling and B7. The higher the deviation from the average GWP, the higher
thermal recycling by means of incineration with energy recovery the flow rate. The flow rate ranges between 6.6 and 9.5 l/min.
of the different materials. Consequently, the production phase has a minor influence on
14 different product types were considered. For the assessment the LCA results.
of the variability of the results, all products were balanced and
7. Requisite evidence
The drinking water regulation determines the quality of drinking • Elastomer guideline: Guideline for the hygienic
water at the point of withdrawal. This results in requirements for assessment of elastomers in contact with drinking water
used materials in drinking water installations in general and • Thermoplastic elastomers: Recommendation for the
therefore in sanitary fittings in particular. hygienic assessment of products made of thermoplastic
All materials used by Hansgrohe SE, which are in contact with elastomers in contact with drinking water (TPE transition
drinking water, fulfill the drinking water regulation. recommendation)
• Ceramics: draft assessment basis for enamels and
Regulations for metals (Europe-wide): ceramic materials: assessment basis for enamels and
ceramic materials in contact with drinking water
• Acceptance of metallic materials used for products in
(enamel/ceramic assessment basis)
contact with drinking water: 4MS Common Approach
• Lubricants: Guideline for the hygienic assessment of
- Part A – Procedure for the acceptance
lubricants in contact with drinking water (sanitary
- Part B – 4MS Common Composition List
lubricants), (Lubricant Guideline)
• Metal recommendation of the federal environment
agency: metal materials suitable for drinking water
Regulation for other materials (France):
hygiene
• ACS: Attestation de Conformité Sanitaire (plastics,
Regulations for other materials (Germany): elastomers)
• KTW: Assessment basis for plastics and other organic
Regulation for other materials (UK):
materials in contact with drinking water
8 Environmental Product Declaration - Hansgrohe Group - Shower Sets - EcoSmart
elastomers)
• BS 69 20: Suitability of non-metallic products for use in
contact with water intended for human consumption with
Products of the Hansgrohe SE are therefore uncritical to use
regard to their effect on the quality of water (plastics,
with any drinking water.
8. References
Standards Draft General administrative provision relating to the Order on
the European list of wastes (Waste List Order – German
EN 1112 designation: AVV) of 10 December 2001.
EN 1112:2008 Sanitary tapware - Shower outlets for sanitary
tapware for water supply systems of type 1 and type 2 - ECHA
General technical specification European Chemicals Agency (ECHA) Candidate List of
Substances of Very High Concern (SVHC) for Authorisation
ISO 3822 https://echa.europa.eu/de/candidate-listtable
ISO 3822: Acoustics – Laboratory tests on noise emission from
appliances and equipment used in water supply installations Ecoinvent
ecoinvent 3.9 Database on Life Cycle Inventories (Life Cycle
DIN 4102-1 Inventory data), ecoinvent Association, Zürich, 2021
DIN 4102-1: Fire behaviour of building materials and building
components - Part 1: Building materials; concepts, EU Ordinance on biocide Products No. 528/2012
requirements and tests. 1998-05 European Parliament, 2012. Regulation (EU) no528/2012 of the
European parliament and of thecouncil of 22 May 2012
DIN EN ISO 9001 concerning the makingavailable on the market and use of
DIN EN ISO 9001:2015: Quality management systems - biocidal products
Requirements (ISO 9001:2015)
Eurostat
DIN EN 13501-1 Eurostat, last update 26/10/2021 on
DIN EN 13501-1:2019-05: Fire classification of construction https://ec.europa.eu/eurostat/databrowser/view/ten00063/default/table?
products and building elements - Part 1:Classification using ang=en
data from reaction to fire tests; German version EN 13501-
1:2018 LCA for Experts
LCA for Experts (GaBi) 10.7, GaBi Software System and
DIN EN ISO 14001 Database for Life Cycle Engineering version 2023.2, Sphera
DIN EN ISO 14001:2015, Environmental management systems Solutions GmbH, Leinfelden-Echterdingen, 1992-2023
— Requirements with guidance for use, 2015- 09
IBU 2021
DIN EN ISO 14025 General Instructions for the EPD programme of Institut Bauen
DIN EN ISO 14025: Environmental labels and declarations - und Umwelt e.V. Version 2.0, Berlin: Institut Bauen und Umwelt
Type III environmental declarations - Principles and procedures, e.V., 2021, www.ibu-epd.com
2011-10
PCR Part A
EN 15804 Institut Bauen und Umwelt e.V. (IBU), Product Category Rules
DIN EN 15804:2012+A2:2019+AC:2021: Sustainability of for Building-Related Products and Services. Part A: Calculation
construction works - Environmental product declarations - Core rules for the life cycle 11 Environmental Product Declaration
rules for the product category of construction products Hansgrohe Group – Hand Showers assessment and
requirements on the project report. Version 2.1, Berlin, 11/2021
DIN EN ISO 45001
DIN EN ISO 45001:2018: Occupational health and safety PCR Part B
management systems — Requirements with guidance for use. Institut Bauen und Umwelt e.V. (IBU), Requirements on the
2018-03 EPD for fittings and showers. Version 1.1, Berlin, 03/2022
DIN EN ISO 50001 Thünen Institute
DIN EN ISO 50001:2018: Energy management systems — Diestel, Sylvia / Weimar, Holger: Der Kohlenstoffgehalt in Holz-
Requirements with guidance for use. 2018-08 und Papierprodukten - Herleitung und Umrechnungsfaktoren.
Thünen Working Paper 38. Johann Heinrich von Thünen-
Further References Institut. Hamburg,
AVV
9 Environmental Product Declaration - Hansgrohe Group - Shower Sets - EcoSmart
Publisher
Institut Bauen und Umwelt e.V. +49 (0)30 3087748- 0
Hegelplatz 1 info@ibu-epd.com
10117 Berlin www.ibu-epd.com
Germany
Programme holder
Institut Bauen und Umwelt e.V. +49 (0)30 3087748- 0
Hegelplatz 1 info@ibu-epd.com
10117 Berlin www.ibu-epd.com
Germany
Author of the Life Cycle Assessment
brands & values GmbH +49 421 70 90 84 33
Hollerallee 14A info@brandsandvalues.com
28209 Bremen www.brandsandvalues.com
Germany
Owner of the Declaration
Hansgrohe Group +49 7836 51-0
Auestr. 5-9 info@hansgrohe-group.com
77761 Schiltach www.hansgrohe-group.com
Germany
10 Environmental Product Declaration - Hansgrohe Group - Shower Sets - EcoSmart
