ENVIRONMENTAL PRODUCT DECLARATION
as per ISO 14025 and EN 15804+A2
Owner of the Declaration Würth Group / Adolf Würth GmbH & Co. KG
Publisher Institut Bauen und Umwelt e.V. (IBU)
Programme holder Institut Bauen und Umwelt e.V. (IBU)
Declaration number EPD-AWU-20230569-CBA1-EN
Issue date 21.03.2024
Valid to 20.03.2029
Stainless Steel screws
Adolf Würth GmbH & Co. KG
www.ibu-epd.com | https://epd-online.com
General Information
Adolf Würth GmbH & Co. KG Stainless Steel screws
Programme holder Owner of the declaration
IBU – Institut Bauen und Umwelt e.V. Würth Group / Adolf Würth GmbH & Co. KG
Hegelplatz 1 Reinhold-Würth Str. 12-17
10117 Berlin 74653 Künzelsau
Germany Germany
Declaration number Declared product / declared unit
EPD-AWU-20230569-CBA1-EN 1 kg weighted average of dowel-type fasteners with thread.
This declaration is based on the product category rules: Scope:
Screws, 01.06.2023 This EPD relates to timber screws, chipboard screws, drilling and tapping
(PCR checked and approved by the SVR) screws, screws for plastics, metric screws and dowel-type fasteners with
thread made of steel or stainless steel. Depending on the type of screw,
these products are generally used for fastening two or more components
Issue date made of wood, steel or plastic.
21.03.2024
The declared environmental data related to 1 kg of stainless steel are
based on a weighted average stainless steel screws in a Würth
manufacturing plant, SWG Schraubenwerk Gaisbach GmbH and
Valid to
internationalized with generic data. The holder of the declaration shall be
20.03.2029 liable for the underlying information and supporting documents; any liability
of IBU (Institut Bauen und Umwelt e. V.) with regard to manufacturer
information, life cycle assessment data and supporting documents is
hereby excluded. The EPD (Environmental Product Declaration) was
created in accordance with EN 15804 + A2: 2022-03. In the following, the
standard is referred to in simplified form as EN 15804.
The owner of the declaration shall be liable for the underlying information
and evidence; the IBU shall not be liable with respect to manufacturer
information, life cycle assessment data and evidences.
The EPD was created according to the specifications of EN 15804+A2. In
the following, the standard will be simplified as EN 15804.
Dipl.-Ing. Hans Peters
(Chairman of Institut Bauen und Umwelt e.V.)
Verification
The standard EN 15804 serves as the core PCR
Independent verification of the declaration and data according to ISO
14025:2011
internally X externally
Florian Pronold Dr.-Ing. Nikolay Minkov,
(Managing Director Institut Bauen und Umwelt e.V.) (Independent verifier)
1 Environmental Product Declaration - Adolf Würth GmbH & Co. KG - Stainless Steel screws
Product
components. Depending on the type of screw, these products
Product description/Product definition are generally used for fastening components made of wood,
Dowel-type fasteners with thread, e.g. screws made of stainless steel or plastic. Possible application examples include timber
steel, are fasteners that can predominantly be used for construction, steel construction, indoor/outdoor use, furniture
fastening two or more components. The materials to be applications or window construction. Examples of Würth
fastened or screw-in surfaces can be made of wood, wood product groups are ASSY, Pias and Piasta screws.
materials, plastic, aluminium, steel, stainless steel or other
metals. Technical Data
Structural data for the respective dowel-type fasteners with
Pin-shaped connectors, such as screws, are generally thread are provided in the corresponding approvals and
manufactured from a wire (stainless steel) and provided with a technical drawings, as shown below in an excerpt from ETA
head on one component side to be tightened. Depending on 11/0190 (ASSY) for wood screws.
the application, it can have different shapes, e.g. countersunk
Constructional data
head, round head, hexagon head or washer head. For
Data based on ASSY plus VG:
anchoring the pin-shaped connectors, a thread is formed on the
opposite side. The thread shape (e.g. wood thread or metric Name Value Unit
thread) is matched to the screw-in surface and can be designed Screw diameter 8 mm
differently in terms of thread height, thread angle or thread Usage category as per ETA 11/0190 -
pitch. The point design of the dowel-type fasteners with thread
Characteristic tension resistance 20 kN
is matched to the application, e.g. wooden tip, drill tip or blunt
Screw length (+1.0/-0.5) 450 - 480 mm
shape. For protection against corrosion or e.g. for setting a
sliding friction, the pin-shaped connectors can be provided with Material carbon steel
different coatings, for example, anti-skid coating. Product according to CPR with hEN:
• Performance values of the product in accordance with
Depending on the application, the additional use of suitable
the declaration of performance in relation to its essential
steel or stainless steel seals as well as EPDM seals (ethylene-
characteristics according to applicable hEN such as EN
propylene-diene rubber), washers or nuts is provided.
15048-1:2016 and EN 14399-1:2015.
Depending on the application, the dowel-type fasteners with
thread can be subject to legal national or European
Product according to CPR with ETA:
requirements such as the Construction Products Regulation.
For example, the following documentation possibilities may be • Performance values of the product according to the
available: declaration of performance with respect to its essential
characteristics in accordance with applicable ETA.
Product according to CPR with hEN:
Regulation (EU) No 305/2011 (CPR) shall apply to the placing Product that is not subject to EU harmonization legislation:
of the product on the market in the EU/EFTA states (with the • Performance values of the product in relation to its
exception of Switzerland). The product requires a declaration of characteristics according to the applicable technical
performance taking into account the respective EN. regulation (no CE marking).
All approvals can be downloaded from the Würth Online Shop
The CE marking shall be applied to the product in compliance homepage under the Documents tab for the respective
with the proof of its conformity with the following harmonized products.
standards based on the mentioned harmonization legislation:
Base materials/Ancillary materials
• EN 14592:2008-04; timber structures - dowel-type
fasteners Dowel-type fasteners with thread are made of stainless steel.
The use shall be subject to the respective national provisions. As explained in the product description (2.1), depending on the
type of application and material, the fasteners are provided
Product according to CPR with ETA: with, for example, galvanic and/or mechanical galvanizing and,
Regulation (EU) No 305/2011 (CPR) shall apply to the placing if appropriate, with anti-friction coating. Depending on the
of the product on the market in the the European application, the fasteners are also equipped with a
Union/European/Free Trade Association (EU/EFTA) states (with corresponding sealing washer made of steel, stainless steel or
the exception of Switzerland). The product needs a declaration aluminium and EPDM sealing rubber.
of performance taking into account the respective ETA such as
ETA-10/0184, ETA-13/0210 or ETA-11/0190 and CE marking. Stainless steel
The designation stainless steel (according to DIN EN 10020)
The use shall be subject to the respective national provisions. refers to alloyed or unalloyed steels with a special degree of
purity, such as steels in which the sulfur and phosphorus
Product that is not subject to EU harmonization content (also known as an iron companion) does not exceed
legislation: 0.025%. Often, additional heat treatments (such as quenching
The national regulations of the place of use apply to the use of and tempering) are planned.
the product. In Germany, for example, the building codes of the
respective countries and the technical building regulations EPDM
based on these codes apply. EPDM is an abbreviation for ethylene-propylene diene
(monomer) rubber and is a terpolymer elastomer (rubber). It
Application thus belongs to the group of synthetic rubbers. In the context of
Timber screws, chipboard screws, drilling and tapping screws, the rubber classification, seals made of this sealing material are
plastic screws and dowel-type fasteners with thread made of therefore assigned to the group of non-polar saturated rubbers.
stainless steel are used when fastening two or more This material is a high-quality rubber-elastic synthetic elastomer
2 Environmental Product Declaration - Adolf Würth GmbH & Co. KG - Stainless Steel screws
of ethylene, propylene and dienes of high-molecular weight. lies on the screw as a dry transparent film. Some lubricating
The saturated basic molecular base structure of EPDM offers coatings contain small amounts of alcohol. Type 6 work
properties such as high weathering resistance, ozone clothing, safety goggles, face protection and chemical-resistant
resistance and high heat resistance. gloves are worn as safety measures to protect human contact
during coating. An annual safety briefing is carried out and
Electrogalvanizing extraction systems are used.
Galvanization (also electroplating technology) is a surface and
coating technology process for the electrochemical separation Reference service life
of metals on metallic or metallized surfaces using an electrolyte Given the wide range of applications, no specific information on
and direct current. Functional electroplating protects against the recommended useful life is provided. The actual service life
corrosion and wear, catalyzes, improves conductivity, and of screws generally depends on their intended use, installation
reduces frictional forces. The ductility and formability of environment and proper installation. External influences can
workpieces can also be influenced by electroplating. have a significant impact on the useful life. According to the
European Technical Approval, the average useful life of screws
Anti-friction coating is > 25 years. The indication of the useful life cannot be
Aqueous suspensions, emulsions and dispersions are used as understood as a guarantee by the manufacturer. It must be
lubricants. Depending on the application, these include ensured that the use of the dowel-type fasteners with thread
kerosenes, polymers and waxes. A lubricious coating is applied complies with the applicable technical regulations.
to the screw by means of an immersion bath or drum coating. It
LCA: Calculation rules
· C1 machine-assisted de- construction (Hand-screwdriver;
Declared Unit battery operated)
1 kg average screws made of stainless steel: · C2 transport to waste processing; 50 km with truck Transport
Declared unit and mass reference distance can be adjusted at building level if necessary (e.g., for
100 km actual transport distance: multiply LCA values by factor
Name Value Unit
2)
Declared unit 1 kg
· C3 waste processing for recycling of Stainless steel.
Gross density 7900 kg/m3 · C4 no components of the product are landfilled.
The exact weight of the screw is provided digitally.
System boundary Benefits and loads beyond the System Boundary (D):
Type of the EPD: cradle-to-gate - with options, modules C1-C4 Module D includes:
and module D (A1-A3 + C + D and additional modules: A4, A5). Material recovery potentials from metal recycling and energy
recovery potentials from the
Production Stage (A1-A3): The Product stage includes: thermal recovery of Packaging.
· A1 Raw material supply and processing (mainly steel),
Geographic Representativeness
· A2 Transport of raw materials to the manufacturer,
Land or region, in which the declared product system is
· A3 Production of Stainless steel screws (incl. energy
manufactured, used or handled at the end of the product´s
provision, treatment of production waste, production of
lifespan: Europe
packaging materials).
Construction stage (A4-A5): The construction process stage Comparability
includes:
Basically, a comparison or an evaluation of EPD data is only
· A4 transport to the construction site 100 km by truck,
possible if all the data sets to be compared were created
· A5 Disposal of the packaging and installation of the Stainless
according to EN 15804 and the building context, respectively
steel screw.
the product-specific characteristics of performance, are taken
into account. The underlying database is LCA FE (GaBi) 2023,
version 2023.1
End-of-life stage (C1-C4): The end-of-life stage includes:
LCA: Scenarios and additional technical information
Characteristic product properties of biogenic carbon
Transport from the gate to the site (A4)
Name Value Unit
Information on describing the biogenic carbon content at
Litres of fuel (per kg transported goods) 0.0018 l/100km
factory gate
Transport distance 100 km
Note: 1 kg of biogenic carbon is equivalent to 44/12 kg of CO2
Capacity utilisation (including empty runs) 61 %
Name Value Unit
Mass for Transportation 1 kg
kg
Biogenic carbon content in product -
C
Assembly (A5)
Biogenic carbon content in accompanying kg
0.0228
packaging C
3 Environmental Product Declaration - Adolf Würth GmbH & Co. KG - Stainless Steel screws
Name Value Unit Reuse, recovery and/or recycling potentials (D), relevant
Electricity consumption 0.0281kWh scenario information
Material loss - kg Name Value Unit
Output substances following waste treatment on collection rate 100 %
0.051 kg
site (Packaging)
The results of the scenario (100%) can be scaled on building
level according to the applied collection rate.
End of life (C1-C4)
Name Value Unit
Energy consumption for dismantling 0.0281 kWh
Collected separately waste type waste type 1 kg
Collected as mixed construction waste - kg
Reuse - kg
Recycling 1 kg
Energy recovery - kg
4 Environmental Product Declaration - Adolf Würth GmbH & Co. KG - Stainless Steel screws
LCA: Results
DESCRIPTION OF THE SYSTEM BOUNDARY (X = INCLUDED IN LCA; MND = MODULE OR INDICATOR NOT DECLARED; MNR
= MODULE NOT RELEVANT)
Benefits and
Construction loads beyond
Product stage Use stage End of life stage
process stage the system
boundaries
la ire ta m w a Ry lp p u s tro p s n a rT g n iru tc a fu n a M e h t m o rf tro p s n a rTe tis e h t o t e ta g y lb m e s s A e s U e c n a n e tn ia M ria p e R tn e m e c a lp e R tn e m h s ib ru fe R y g re n e la n o ita re p Oe s u re ta w la n o ita re p Oe s u n o itc u rts n o c -e Dn o itilo m e d tro p s n a rT g n is s e c o rp e ts a W la s o p s iD -e s u e R-y re v o c e R-g n ilc y c e Rla itn e to p
A1 A2 A3 A4 A5 B1 B2 B3 B4 B5 B6 B7 C1 C2 C3 C4 D
X X X X X MND MND MNR MNR MNR MND MND X X X X X
RESULTS OF THE LCA - ENVIRONMENTAL IMPACT according to EN 15804+A2: 1 kg Stainless steel fasteners with thread
Parameter Unit A1-A3 A4 A5 C1 C2 C3 C4 D
GWP-total kg CO 2 eq 6.88E+00 6.69E-03 1.2E-01 4.26E-02 4.34E-03 0 0 -4.31E+00
GWP-fossil kg CO 2 eq 6.94E+00 6.61E-03 4.5E-02 4.26E-02 4.29E-03 0 0 -4.32E+00
GWP-biogenic kg CO 2 eq -7.44E-02 1.95E-05 7.55E-02 2.12E-05 1.27E-05 0 0 1.98E-02
GWP-luluc kg CO 2 eq 1.52E-02 6.13E-05 4.29E-06 3.9E-06 3.98E-05 0 0 -1.14E-02
ODP kg CFC11 eq 6.76E-12 8.61E-16 4.28E-13 4.19E-13 5.59E-16 0 0 -1.76E-13
AP mol H+ eq 3.92E-02 9.86E-06 8.37E-05 6.49E-05 6.4E-06 0 0 -2.63E-02
EP-freshwater kg P eq 1.43E-05 2.42E-08 4.48E-08 4.21E-08 1.57E-08 0 0 -6.21E-06
EP-marine kg N eq 6.88E-03 3.6E-06 2.52E-05 1.83E-05 2.34E-06 0 0 -3.78E-03
EP-terrestrial mol N eq 7.46E-02 4.25E-05 2.79E-04 1.93E-04 2.76E-05 0 0 -4.09E-02
kg NMVOC
POCP 1.99E-02 8.66E-06 6.87E-05 5.06E-05 5.62E-06 0 0 -1.15E-02
eq
ADPE kg Sb eq 2.34E-04 4.36E-10 2.14E-09 2.06E-09 2.83E-10 0 0 -6.3E-06
ADPF MJ 7.45E+01 9.01E-02 9.58E-01 9.36E-01 5.85E-02 0 0 -5.27E+01
m3 world eq
WDP 2.26E+00 7.99E-05 1.21E-02 3.58E-03 5.19E-05 0 0 -1.75E+00
deprived
GWP = Global warming potential; ODP = Depletion potential of the stratospheric ozone layer; AP = Acidification potential of land and water; EP =
Eutrophication potential; POCP = Formation potential of tropospheric ozone photochemical oxidants; ADPE = Abiotic depletion potential for non-fossil
resources; ADPF = Abiotic depletion potential for fossil resources; WDP = Water (user) deprivation potential)
RESULTS OF THE LCA - INDICATORS TO DESCRIBE RESOURCE USE according to EN 15804+A2: 1 kg Stainless steel
fasteners with thread
Parameter Unit A1-A3 A4 A5 C1 C2 C3 C4 D
PERE MJ 1.37E+01 6.56E-03 9.97E-01 1.28E-01 4.26E-03 0 0 -9.94E+00
PERM MJ 8.64E-01 0 -8.64E-01 0 0 0 0 0
PERT MJ 1.45E+01 6.56E-03 1.33E-01 1.28E-01 4.26E-03 0 0 -9.94E+00
PENRE MJ 7.46E+01 9.04E-02 9.72E-01 9.36E-01 5.87E-02 0 0 -5.28E+01
PENRM MJ 1.38E-02 0 -1.38E-02 0 0 0 0 0
PENRT MJ 7.46E+01 9.04E-02 9.58E-01 9.36E-01 5.87E-02 0 0 -5.28E+01
SM kg 2.49E-01 0 0 0 0 0 0 7.61E-01
RSF MJ 0 0 0 0 0 0 0 0
NRSF MJ 0 0 0 0 0 0 0 0
FW m3 8.19E-02 7.18E-06 4.15E-04 2.15E-04 4.66E-06 0 0 -7.17E-02
PERE = Use of renewable primary energy excluding renewable primary energy resources used as raw materials; PERM = Use of renewable primary
energy resources used as raw materials; PERT = Total use of renewable primary energy resources; PENRE = Use of non-renewable primary energy
excluding non-renewable primary energy resources used as raw materials; PENRM = Use of non-renewable primary energy resources used as raw
materials; PENRT = Total use of non-renewable primary energy resources; SM = Use of secondary material; RSF = Use of renewable secondary fuels;
NRSF = Use of non-renewable secondary fuels; FW = Use of net fresh water
RESULTS OF THE LCA – WASTE CATEGORIES AND OUTPUT FLOWS according to EN 15804+A2:
1 kg Stainless steel fasteners with thread
Parameter Unit A1-A3 A4 A5 C1 C2 C3 C4 D
HWD kg 1.76E-06 2.8E-13 5.49E-11 5.43E-11 1.82E-13 0 0 -4.8E-04
NHWD kg 3.65E+00 1.38E-05 2.41E-03 2.06E-04 8.95E-06 0 0 4.68E-02
RWD kg 1.08E-03 1.69E-07 1.47E-04 1.46E-04 1.1E-07 0 0 -3.73E-04
CRU kg 0 0 0 0 0 0 0 0
MFR kg 1.02E-02 0 0 0 0 1E+00 0 0
MER kg 0 0 0 0 0 0 0 0
EEE MJ 0 0 1.04E-01 0 0 0 0 0
5 Environmental Product Declaration - Adolf Würth GmbH & Co. KG - Stainless Steel screws
EET MJ 0 0 1.89E-01 0 0 0 0 0
HWD = Hazardous waste disposed; NHWD = Non-hazardous waste disposed; RWD = Radioactive waste disposed; CRU = Components for re-use;
MFR = Materials for recycling; MER = Materials for energy recovery; EEE = Exported electrical energy; EET = Exported thermal energy
RESULTS OF THE LCA – additional impact categories according to EN 15804+A2-optional:
1 kg Stainless steel fasteners with thread
Parameter Unit A1-A3 A4 A5 C1 C2 C3 C4 D
Disease
PM 6.13E-07 8.16E-11 6.9E-10 5.87E-10 5.3E-11 0 0 -5.68E-07
incidence
IR kBq U235 eq 1.1E-01 2.52E-05 2.21E-02 2.19E-02 1.64E-05 0 0 -4.19E-02
ETP-fw CTUe 2.32E+01 6.4E-02 2.78E-01 2.68E-01 4.16E-02 0 0 -3.15E+01
HTP-c CTUh 1.34E-06 1.31E-12 5.41E-12 4.84E-12 8.5E-13 0 0 -6.4E-08
HTP-nc CTUh 1.46E-07 6.98E-11 2.71E-10 2.48E-10 4.53E-11 0 0 -3.26E-08
SQP SQP 3.43E+01 3.76E-02 1.33E-01 1.27E-01 2.44E-02 0 0 -7.26E+00
PM = Potential incidence of disease due to PM emissions; IR = Potential Human exposure efficiency relative to U235; ETP-fw = Potential comparative
Toxic Unit for ecosystems; HTP-c = Potential comparative Toxic Unit for humans (cancerogenic); HTP-nc = Potential comparative Toxic Unit for humans
(not cancerogenic); SQP = Potential soil quality index
Disclaimer 1 – for the indicator “Potential Human exposure efficiency relative to U235”. This impact category deals mainly with the
eventual impact of low-dose ionizing radiation on human health of the nuclear fuel cycle. It does not consider effects due to possible
nuclear accidents, occupational exposure or radioactive waste disposal in underground facilities. Potential ionizing radiation from the
soil, radon and from some construction materials is also not measured by this indicator.
Disclaimer 2 – for the indicators “abiotic depletion potential for non-fossil resources”, “abiotic depletion potential for fossil resources”,
“water (user) deprivation potential, deprivation-weighted water consumption”, “potential comparative toxic unit for ecosystems”,
“potential comparative toxic unit for humans – cancerogenic”, “Potential comparative toxic unit for humans - not cancerogenic”,
“potential soil quality index”. The results of this environmental impact indicator shall be used with care as the uncertainties on these
results are high as there is limited experience with the indicator.
References
Standards: Leinfelden Echterdingen
EN 15804
EN 15804:2012+A1 2013, Sustainability of construction works GaBi documentation
— Environmental Product Declarations — Core rules for the LCAFE (GaBI) life cycle inventory data documentation
product category of construction products. (http://www.gabi-software.com/international/databases/gabi-
data-search/)
EN 15804
EN 15804:2012+A2:2019+AC:2021, Sustainability of IBU 2021
construction works — Environmental Product Declarations — Institut Bauen und Umwelt e.V.: General Programme
Core rules for the product category of construction products. Instructions
for the Preparation of EPDs at the Institut Bauen und Umwelt
EN 14592 e.V., version 2.0., Berlin: Institut Bauen und Umwelt e.V., 2021,
EN 14592:2008-04, Timberstructures– Dowel-typefasteners– http://www.ibu-epd.com
Requirements
PCR Part A
ISO 14025 Calculation Rules for the Life Cycle Assessment and
EN ISO 14025:2011, Environmental labels and declarations — Requirements on the Project
Type III environmental declarations — Principles and Report,Berlin: Institut Bauen und Umwelt e.V., www.ibu-
procedures. epd.com, Version 1.3, 2021
DIN EN 10020 PCR Part B
DIN EN 10020:2000, Definition and classification of grades of Requirements on the EPD for Screws ,
steel version 8, Institut Bauen und Umwelt e.V., www.bau-
umwelt.com, 2023
Literature: ETA-11/0190 (ASSY)
LCAFE (GaBI) software
Sphera Solutions GmbH ETA-10/0184
LCAFE (GaBI) Software
System and Database for Life Cycle Engineering ETA-13/0210
CUP Version: 2023.1
University of Stuttgart Regulation (EU) No 305/2011 (CRB)
6 Environmental Product Declaration - Adolf Würth GmbH & Co. KG - Stainless Steel screws
Publisher
Institut Bauen und Umwelt e.V. +49 (0)30 3087748- 0
Hegelplatz 1 info@ibu-epd.com
10117 Berlin www.ibu-epd.com
Germany
Programme holder
Institut Bauen und Umwelt e.V. +49 (0)30 3087748- 0
Hegelplatz 1 info@ibu-epd.com
10117 Berlin www.ibu-epd.com
Germany
Author of the Life Cycle Assessment
Sphera Solutions GmbH +49 711 341817-0
Hauptstraße 111- 113 info@sphera.com
70771 Leinfelden-Echterdingen www.sphera.com
Germany
Owner of the Declaration
Würth Group / Adolf Würth GmbH & Co. KG +49 7940 15-0
Reinhold-Würth Str. 12-17 info@wuerth.com
74653 Künzelsau www.wuerth.com
Germany
Adolf Würth GmbH & Co. KG +49 7940/15-0
Reinhold-Würth-Str. 12-17 info@wuerth.com
74653 Künzelsau www.wuerth.de
Germany
Würth Industrie Service GmbH & Co. KG +49 7931 91-0
Industriepark Würth, Drillberg - info@wuerth-industrie.com
97980 Bad Mergentheim www.wuerth-industrie.com
Germany
7 Environmental Product Declaration - Adolf Würth GmbH & Co. KG - Stainless Steel screws
