ENVIRONMENTAL PRODUCT DECLARATION
as per ISO 14025 and EN 15804+A1
Owner of the Declaration Sto SE & Co. KGaA
Programme holder Institut Bauen und Umwelt e.V. (IBU)
Publisher Institut Bauen und Umwelt e.V. (IBU)
Declaration number EPD-IWM-STO-20210130-IBG1-DE
Issue date 07.07.2021
Valid to 06.07.2026
Mineral pre-made mortar: rendering mortar – Reinforcement
Fibre Plaster
Sto SE & Co. KGaA
www.ibu-epd.com | https://epd-online.com
Umwelt Produktdeklaration Name des Herstellers – Name des Produkts
1. General Information
Sto SE & Co. KGaA Rendering mortar – Reinforcement
Fibre Plaster
Programme holder Owner of the declaration
IBU – Institut Bauen und Umwelt e.V. Sto SE & Co. KGaA
Panoramastr. 1 Ehrenbachstraße 1
10178 Berlin D-79780 Stühlingen
Germany Germany
Declaration number Declared product / declared unit
EPD-IWM-STO-20210130-IBG1-DE 1 kg rendering mortar as a mineral pre-made mortar,
Reinforcement Fibre Plaster product group with a dry
bulk density less than 1600 kg/m³.
Product names:
Sto-Systemputz, Sto Systemputs, Sto Systemputs, Sto
Systempuds, Sto Verkotuslaasti, (DE, SE, NO, DK, FI);
Sto Sockelputz, Sto Sockelputs, Sto Sockelputs, Sto
Sockelpuds, Sto Sokkelilaasti, (DE, SE, NO, DK, FI);
Sto-Systemputz SF, Sto Verkotuslaasti SF, (DE, FI);
StoLevell Evo, (DE, SE, NO, DK, FI);
This declaration is based on the product Scope:
category rules: This document is a model EPD. When calculating the
Mineral factory-made mortar, 11.2017 Life Cycle Assessment, the product selected to
(PCR checked and approved by the SVR) represent the group in question was the product with
the highest environmental impact in that group. This
EPD applies exclusively to rendering and plastering
Issue date
mortars – Reinforcement Fibre Plaster as mineral pre-
07.07.2021
made mortars for association members; these can be
found on the association’s website. Any numerical
Valid to values – e.g. for constructional data or concentration
06.07.2026 specifications – are average values that are customary
in practice for this product group.
The owner of the declaration shall be liable for the
underlying information and evidence; the IBU shall not
be liable with respect to manufacturer information, life
cycle assessment data and evidences.
The EPD was created according to the specifications
of EN 15804+A1. In the following, the standard will be
simplified as EN 15804.
Verification
The standard EN 15804 serves as the core PCR
Independent verification of the declaration and data
according to ISO 14025:2010
Dipl. Ing. Hans Peters internally x externally
(chairman of Institut Bauen und Umwelt e.V.)
Dr. Alexander Röder Matthias Schulz
(Managing Director Institut Bauen und Umwelt e.V.)) (Independent verifier)
2. Product
2.1 Product description/Product definition Mineral rendering and plastering mortars are mixtures
Mineral pre-made mortars are mortars whose of one or more mineral binders, aggregates, water, and
components are mixed at the factory and not on the – if applicable – additions or admixtures for the
construction site. They are divided into three different manufacture of renders or plasters. Rendering and
types – masonry mortar, rendering and plastering plastering mortars are applied to walls and ceilings in
mortar, and screed material – depending on the type of one or more layers as required. Alongside the
application. aesthetic design of the surface, they protect against
effects of the weather when used as external renders
2 Environmental Product Declaration Sto SE & Co. KGaA – Mineral pre-made mortar: rendering mortar – Reinforcement
Fibre Plaster
and provide an even substrate for paint coats and 2.4 Delivery status
wallpaper when used as internal plasters. In the case Mineral rendering and plastering mortars –
of reinforced concrete ceilings and stairs, Reinforcement Fibre Plaster are produced and
renders/plasters also serve as fire protection; when delivered as pre-made dry mortars. Pre-made dry
porous aggregates are added, they serve as thermal mortar is a mortar made from raw materials that are
protection. Depending on the technical data, the base placed into containers dry at the factory, delivered to
materials and processing aids used, and the practical the construction site, and then mixed with the required
application, rendering and plastering mortars are quantity of water to form ready-to-use mortar based on
divided into the following product groups: the manufacturer’s instructions and conditions.
normal/finishing render or plaster, normal/finishing Delivered in sacks up to 35 kg per sack or in silos up to
render, or plaster with special properties, lightweight 15 t per silo.
render, Reinforcement Fibre Plaster, and insulating
render with an especially high proportion of lightweight 2.5 Base materials/Ancillary materials
aggregates.
Placing Reinforcement Fibre Plaster on the market in Mineral building products such as mineral pre-made
the EU/EFTA (with the exception of Switzerland) is mortars and rendering and plastering mortars mainly
subject to Regulation (EU) No. 305/2011 (CPR). consist of abundant mineral raw materials. Scarcity of
Reinforcement Fibre Plaster requires a declaration of resources is not an issue.
performance – taking into consideration DIN EN 998- Name Value Unit
1:2017-02, Specification for mortar for masonry - Part Aggregate 30-40 M.-%
1: Rendering and plastering mortar – and the CE Fine aggregate 20-25 M.-%
marking. Lightweight aggregate ≤ 10 M.-%
The relevant national regulations apply with regard to Artificial lightweight aggregate - M.-%
usage. Cement 25-35 M.-%
Hydrated lime [Ca(OH2] - M.-%
2.2 Application
Rendering and plastering mortars produced in the The permissible fluctuation range of the constructional
factory for use as a base coat or finishing data is enabled by the variety of proportions of base
render/plaster on walls, ceilings, piers, and separating materials. In each case, the composition of the
walls of structures which comply with the applicable rendering and plastering mortars adds up to 100 m%.
standards or on similar backgrounds (e.g. in the case The following processing aids and admixtures can be
of existing buildings). used as needed:
Reinforcement Fibre Plaster as an inlay plaster for the
 Synthetic dispersion: < 4.00 m%
production of internal plaster and external render on
 Water retention agent: < 0.30 m%
difficult plaster substrates.
 Air entraining admixture: < 0.05 m%
2.3 Technical Data  Thickening agent: < 0.06 m%
 Mineral pigments: < 0.20 m%
 Fibres: < 0.25 m%
Constructional data
 Hydrophobic agent: < 0.45 m%
Name Value Unit
Compressive strength in Aggregate: Natural sands as natural raw materials,
1.5 - 7.5 N/mm2
accordance with DIN EN 1015-11 which contain natural minor and trace minerals along
Thermal conductivity in with the main minerals quartz (SiO2) or calcite
accordance with DIN EN 1745 ≤ 0,61 W/(mK) (CaCo3).
lambda10,dry,mat / P = 50 % Fine aggregate: Limestone dusts which arise as a
Thermal conductivity in result of the preparation of natural sand for the
accordance with DIN EN 1745 ≤ 0,66 W/(mK) production of aggregates, as well as ultra-fine sands.
lambda10,dry,mat / P = 90 % Lightweight aggregate: Natural or artificial mineral
Sound absorption coefficient (as lightweight aggregates for reducing the dry bulk
- %
required) density. Natural lightweight aggregates are
Water-vapour transmission rate in manufactured from natural raw materials via grinding
15/35 -
accordance with DIN EN 1015-19 (e.g. pumice or vermiculite). Artificial lightweight
Dry bulk density in accordance aggregates are manufactured by processing, melting,
≤ 1600 kg/m³
with DIN EN 1015-10 and swelling suitable natural raw materials (swelling
Capillary absorption in accordance kg/(m²min clay, perlite) or sorted recycled glass (expanded
n/a
with DIN EN 1015-18 ^0,5) glass).
Artificial lightweight aggregate: Organic, expanded
polystyrene (EPS) produced by foaming in spherical or
Performance values of Reinforcement Fibre Plaster particle form (recycled) for reducing the dry bulk
according to the declaration of performance in relation density.
to its key characteristics in accordance with DIN EN Cement: As per DIN EN 197-1; cement is used as a
998-1:2017-02, Specification for mortar for masonry - binder and is mainly made from limestone marl or a
Part 1: Rendering and plastering mortar. mixture of limestone and clay. The natural raw
Adhesive shear strength, bond strength, and flexural materials are baked and then ground.
strength are not relevant. Hydrated lime: As per DIN EN 459; white hydrated
lime is used as a binder and is made by baking natural
limestone followed by slaking.
3 Environmental Product Declaration Sto SE & Co. KGaA – Mineral pre-made mortar: rendering mortar – Reinforcement
Fibre Plaster
Synthetic dispersion: Polymer powder for improving
the adhesive bond, elasticity, mechanical properties,
etc. in thin-bed mortar.
Water retention agent: Cellulose ether, made from
cellulose, which prevents dehydration from occurring in
the fresh mortar too quickly.
Air entraining admixture: Surfactants for reducing
the surface tension of water and producing entrained
air. This reduces the bulk density of fresh mortar,
improves workability, and reduces the tendency
towards contraction and stress cracking.
Thickening agent: Cellulose or starch ether, made
from cellulose or crystal starch, improves the
resistance to flow, and thus has a thickening effect, but
does not have any water-retaining properties.
Mineral pigments: Natural or synthetic powder-form
colouring materials which are produced by mechanical
processing of the relevant mineral substances such as
chalk, clay, etc.
Graphic 1: Manufacturing process (green: input; blue:
Fibres: Fibres from natural or synthetic polymers (e.g.
unit process)
PAN, PP, PE, etc.) or mineral chemical fibres (e.g.
glass fibres) are used to absorb tensile forces in solid
2.7 Environment and health during
mortar.
manufacturing
Hydrophobic agent: Water-soluble sodium oleate or
The current state of the art includes the 100 % return
zinc stearate for reducing the capillary absorption of
of dry waste into production. In all places where dust
the solid mortar.
can arise during production in the factory, this waste is
fed into a central filter system using the appropriate
Information about Substances of Very High Concern:
extraction systems, taking into account the
The product contains substances from the ECHA
occupational limit values. The very fine dust filtered out
candidate list (15.01.2019) above 0.1 % w/w: no.
in these systems is then fed back into the
The product contains further CMR substances from
manufacturing process. As part of the quality
Category 1A or 1B which are not on the candidate list
management systems introduced, any off-specification
above 0.1 % w/w in at least one part of the product: no.
batches are detected immediately by the automated
Biocide products have been added to this building
process monitoring system and are fed into circulation
product or it has been treated with biocide products
via appropriate recovered-goods silos, i.e. they are fed
(thus it is a treated product in the sense of the Biocide
back into the production process in very small
Products Ordinance (EU) No. 528/2012): no
quantities. This procedure is also applied for product
residues which are transported back to the
2.6 Manufacture
manufacturing plant in small quantities in silos or
The graphic shows the manufacturing process.
sacks.
Mineral rendering and plastering mortars are made in
Process exhaust air is dedusted until the level is far
mixing plants in the following steps:
below the statutory occupational limit values.
 Filling of the storage or weighing containers
 Conveyance of ingredients and substances Noise:
being mixed into the mixer Noise level measurements have shown that all values
determined inside and outside the production facilities
 Mixing
are well below the required specifications of the
 Conveyance of finished products
technical standards thanks to noise protection
 Packaging measures being taken.
 Loading and shipping of the finished product
2.8 Product processing/Installation
Mineral rendering and plastering mortars are normally
The raw materials – sand, binder, lightweight
applied by machine. They are extracted from the silo
aggregates, processing aids, admixtures, and
with a dry-materials conveying machine or from
additions (see base materials) – are stored at the
individual containers and mixed with a mixing pump
manufacturing plant in silos. From the silos, the raw
before being conveyed and applied. Silo mixing pumps
materials are gravimetrically dosed and intensely
can also be used. Reinforcement Fibre Plaster can
mixed according to the respective formulation. The
also be mixed by hand. The rendering and plastering
mixture is then packaged and shipped dry as pre-made
mortars are then levelled, and textured if necessary, on
dry mortar in containers or silos.
site with suitable tools. The regulations of the
employers’ liability insurance associations and the
respective safety data sheets of the building products
apply.
With the cement and lime binders in mineral pre-made
mortars, the fresh mortar mixed with water is strongly
alkaline. Prolonged contact can cause serious skin
damage owing to the alkalinity. Personal protective
measures must therefore be taken (EU Health &
Safety Data Sheet) to avoid any contact with eyes or
skin.
4 Environmental Product Declaration Sto SE & Co. KGaA – Mineral pre-made mortar: rendering mortar – Reinforcement
Fibre Plaster
No special measures are required for protection of the class A1 is always verified with a test as a matter of
environment. Unchecked dust emissions must be course.
avoided. Reinforcement Fibre Plaster is often used in external
Mineral pre-made mortars must not enter the sewer wall insulation systems approved by general building
system, surface water, or ground water. inspection requirements. The tests required in terms of
fire protection are always carried out on the entire
2.9 Packaging system. The reaction to fire of Reinforcement Fibre
Bagged cargo from a paper bag with a plastic insert, Plaster is usually equivalent to or better than the
sacks stored on wooden pallets, pallets wrapped in approved system.
plastic film, silo-based goods stored in steel silos. Regardless of the product group, it has been shown in
Possibilities of reuse for the packaging of bagged the “hot” measurement (structural analysis with the
cargo – separation if necessary. Unsoiled polythene resistance of the masonry reduced under the influence
films (correct sorting must be applied) and reusable of fire temperatures) that rendering and plastering
wooden pallets are taken back by the building material mortar made from mineral pre-made mortars has a
dealer (reusable wooden pallets subject to beneficial effect on the required minimum wall
reimbursement as per the deposit system), returned to thickness.
the mortar plants by the dealer, and fed back into the Depending on the product, additional labels will appear
production process. The films are forwarded to the film on containers with the CE mark or declaration of
manufacturers for recycling. performance.
Fire protection
2.10 Condition of use Name Value
The specified products are rot-resistant and ageing- Building material class A1
resistant during normal use that conforms to the Burning droplets -
intended purpose of the products described. Smoke gas development -
Rendering and plastering mortars made from mineral
pre-made mortars must be protected from long-term Water
weather effects, e.g. by properly connecting the facade Mineral pre-made mortars as rendering and plastering
plinth (SAF). mortars are structurally stable and are not subject to
The cracking resistance of rendering and plastering changes in shape as a result of water exposure and
mortars made from mineral pre-made mortars can be drying.
increased with cracking reinforcement in the tension-
stressed areas of the render (DIN EN 13914-1, -2, DIN Mechanical destruction
18550-1, -2). No specifications required.
2.11 Environment and health during use 2.14 Re-use phase
Due to the stable calcium silicate hydrate (CSH) The service life of masonry coated with Reinforcement
adhesion and the firm structures achieved through Fibre Plaster normally ends along with the service life
curing on the substrate, emissions are rendered of the simultaneously erected building. Reuse and
impossible. During normal use conforming to the further use of masonry coated with render after
intended purpose of the products described, any demolition is not possible.
adverse health effects have been rendered impossible. Elements of building construction made from mineral
No hazards for water, air, and soil are known for use rendering and plastering mortars can normally be
as per the intended application of the products. stripped down easily. During demolition of a building,
The natural ionising radiation of the rendering and these elements do not have to be treated as special
plastering mortars made from mineral pre-made waste, but the sorting during demolition must be as
mortars is extremely low and does not pose any exact as possible. Mineral rendering and plastering
health-related risks. mortars can be recycled as building materials. They
are normally reused in structural and civil engineering
2.12 Reference service life in the form of recycled aggregates.
A reference service life (RSL) as per ISO 15686-1, -2, -
7, and -8 is not declared. Provided they are used as 2.15 Disposal
intended and properly applied, the service life of Mortar is categorised as mineral construction waste.
rendering and plastering mortars made from mineral 78.4 % of construction waste is recycled. German
pre-made mortars on walls and ceilings has been Building Materials Association
known to be 40 years or longer (BBSR). The suitability of hardened mineral rendering and
plastering mortars for landfill as per landfill class I is
ensured according to the Technical Instruction on
2.13 Extraordinary effects Municipal Waste (TASi). The EWC waste code
according to the waste reuse directory is 170101.
Fire
Fire protection class A1 2.16 Further information
Further information is available online at
Because the proportion of finely dispersed organic www.vdpm.info.
components is greater than 1 %, the fire protection
3. LCA: Calculation rules
5 Environmental Product Declaration Sto SE & Co. KGaA – Mineral pre-made mortar: rendering mortar – Reinforcement
Fibre Plaster
3.1 Declared Unit All of the background records relevant to the
This declaration refers to the production of one assessment have been retrieved from the GaBi8
kilogram of typical rendering and plastering mortar of database, with the exception of the pumice
the Reinforcement Fibre Plaster product group. Only (ROTOCELL) record.
dry mortars are taken into consideration.
3.6 Data quality
Specification of declared unit Representative products were used for this model EPD
– the product with the greatest environmental impact
Name Value Unit was declared to be representative of a group in order
Declared unit 1 kg to calculate the Life Cycle Assessment results.
Gross density ≤ 1600 kg/m3 Corresponding background records were available in
Spreading rate 0,80-0,95 l/kg the GaBi database for all relevant primary products
Conversion factor to 1 kg 1 - used.
The requirements in terms of data quality and
The product which demonstrates the highest background data correspond to the specifications of
environmental impact of the Reinforcement Fibre PCR Part A.
Plaster product group is selected from that group for The technological background of the data collected
calculating the Life Cycle Assessment. reflects the physical reality for the declared product
group.
The records are complete and fulfil the system
3.2 System boundary boundaries and criteria for the exclusion of inputs and
The life cycle analysis of the products being examined outputs.
encompasses the production of the mortar including The last audit of the data used was less than 8 years
raw material extraction and the provision of energy ago.
sources up to the packaged, finished product (module
A1-A3), the application of the product including 3.7 Period under review
transportation to the construction site (module A4-A5), The period under review is one year of production
the usage phase (module B1), and disposal of the based on the year 2018. The reference area of the Life
mortar (module C4). For silo-based goods, the Cycle Assessments was limited to Germany. The
proportionate expenditure for transportation and result is that, besides production processes under
manufacturing of the silo is taken into account. Credit these marginal conditions, the precursors also relevant
for packaging including energy recovery (module D) is for Germany, such as electricity and energy provision,
also incorporated into the Life Cycle Assessment. were used.
3.8 Allocation
3.3 Estimates and assumptions Specific information on the allocations within the
For the individual formulation components of the background records can be found in the
formulations, these were assessed according to documentation of the GaBi records. The material and
manufacturer specifications or literature in the event energy consumption for the declared product were
that no specific GaBi 8 processes were available. allocated by the member companies of the VDPM. The
data made available consists of internal key figures
3.4 Cut-off criteria which have not been published. A multi-input allocation
At the input side, all material flows that enter the is used as per a simple credit method with a credit for
system and are greater than 1 % of their total mass or power and thermal energy when burning packaging
contribute more than 1 % to primary energy demand and production waste as well as the landfilling of
are taken into consideration. The total amount of input production waste. The credit from the disposal of
flows not taken into consideration is maximum 5 % of packaging is credited in module D.
the energy and mass in use.
The manufacturing of the machines, facilities, and 3.9 Comparability
other infrastructure required for the production of the Basically, a comparison or an evaluation of EPD data
relevant products was not taken into consideration for is only possible if all the data sets to be compared
the Life Cycle Assessments. were created according to EN 15804 and the building
context, respectively the product-specific
3.5 Background data characteristics of performance, are taken into account.
The software system GaBi8 was used for modelling
the life cycle for the production of the mortar products. The GaBi 8 background database was used for
modelling purposes.
4. LCA: Scenarios and additional technical information
The following technical information is necessary for the empty runs)
declared modules or can be used for the development Gross density of products
1600 kg/m3
of specific scenarios in the context of building transported
assessment if modules have not been declared (MND).
Transportation to the construction site (A4) Installation in the building (A5)
Name Value Unit Name Value Unit
Litres of fuel 0.0063 l/100km Auxiliary 0 kg
Transport distance 300 km Water consumption 0.0003 m3
Capacity utilisation (including 50 - 85 % Other resources 0 kg
6 Environmental Product Declaration Sto SE & Co. KGaA – Mineral pre-made mortar: rendering mortar – Reinforcement
Fibre Plaster
Electricity consumption 0.00045 kWh
Other energy carriers 0 MJ
Material loss 0 kg
Output substances following
0 kg
waste treatment on site
Dust in the air 0 kg
VOC in the air 0 kg
For use (B1) see Chapter 2.12 on use
In the use stage, the carbon dioxide absorbed by
means of carbonation is taken into consideration. The
carbon dioxide released during the neutralisation of
limestone (CaCO3) in the production of lime and
cement is reabsorbed when reacting with the lime and
cement binders, thus leading to an increase in
strength. In line with DIN EN 16757, the resulting
maximum theoretical carbon dioxide absorption for
fully carbonated rendering and plastering mortars and
the practical total maximum potential for carbon
dioxide absorption – taking into account the degree of
exposure of the surfaces – were calculated in the Life
Cycle Assessment of the pre-made mortar.
End of the life cycle (C1-C4)
Name Value Unit
Collected separately Abfalltyp 0 kg
Collected as mixed construction
0 kg
waste
Reuse 0 kg
Recycling 0 kg
Energy recovery 0 kg
Landfilling 1.12 kg
Reuse, recovery, and recycling potential (D);
relevant scenario specifications
Name Value Unit
Recycling Silo (packaging) 100 %
Burning of wooden pallets
100 %
(packaging)
Burning of paper (packaging) 100 %
Burning of polythene film
100 %
(packaging)
7 Environmental Product Declaration Sto SE & Co. KGaA – Mineral pre-made mortar: rendering mortar – Reinforcement
Fibre Plaster
5. LCA: Results
DESCRIPTION OF THE SYSTEM BOUNDARY (X = INCLUDED IN LCA; MND = MODULE NOT DECLARED;
MNR = MODULE NOT RELEVANT)
BENEFITS AND
CONSTRUCTI LOADS
PRODUCT STAGE ON PROCESS USE STAGE END OF LIFE STAGE BEYOND THE
STAGE SYSTEM
BOUNDARIES
8 Environmental Product Declaration Sto SE & Co. KGaA – Mineral pre-made mortar: rendering mortar – Reinforcement
Fibre Plaster
lairetam
waR
ylppus tropsnarT
gnirutcafunaM
eht
morf
tropsnarT
etis
eht
ot
etag
ylbmessA esU
ecnanetniaM
riapeR
tnemecalpeR tnemhsibrufeR
ygrene
lanoitarepO esu
retaw
lanoitarepO esu
noitcurtsnoc-eD
noitilomed tropsnarT
gnissecorp
etsaW
lasopsiD -esueR -yrevoceR -gnilcyceR laitnetop
A1 A2 A3 A4 A5 B1 B2 B3 B4 B5 B6 B7 C1 C2 C3 C4 D
X X X X X X MND MNR MNR MNR MND MND MND MND MND X X
RESULTS OF THE LCA - ENVIRONMENTAL IMPACT according to EN 15804+A1: 1 kg Reinforcement
Fibre Plaster
Parameter Unit A1-A3 A4 A5 B1 C4 D
Global warming potential [kg CO2-Eq.] 4.33E-1 2.19E-2 4.77E-2 -1.47E-1 1.79E-2 -1.98E-2
Depletion potential of the stratospheric ozone layer [kg CFC11-Eq.] 3.01E-9 4.59E-16 6.32E-16 0.00E+0 3.97E-15 -1.45E-14
Acidification potential of land and water [kg SO2-Eq.] 8.27E-4 1.67E-5 6.19E-6 0.00E+0 1.06E-4 -2.13E-5
Eutrophication potential [kg (PO4)3--Eq.] 1.46E-4 3.75E-6 1.37E-6 0.00E+0 1.46E-5 -3.52E-6
Formation potential of tropospheric ozone photochemical
[kg ethene-Eq.] 9.44E-5 -2.36E-7 4.13E-7 0.00E+0 8.20E-6 -1.86E-6
oxidants
Abiotic depletion potential for non-fossil resources [kg Sb-Eq.] 1.35E-6 2.27E-9 8.17E-10 0.00E+0 6.86E-9 -2.99E-8
Abiotic depletion potential for fossil resources [MJ] 4.30E+0 2.93E-1 1.23E-2 0.00E+0 2.31E-1 -2.55E-1
RESULTS OF THE LCA - INDICATORS TO DESCRIBE RESOURCE USE according to EN 15804+A1: 1 kg
Reinforcement Fibre Plaster
Parameter Unit A1-A3 A4 A5 B1 C4 D
Renewable primary energy as energy carrier [MJ] 5.63E-1 1.98E-2 3.30E-1 0.00E+0 2.97E-2 -5.96E-2
Renewable primary energy resources as material utilization [MJ] 3.27E-1 0.00E+0 -3.27E-1 0.00E+0 0.00E+0 0.00E+0
Total use of renewable primary energy resources [MJ] 8.90E-1 1.98E-2 2.62E-3 0.00E+0 2.97E-2 -5.96E-2
Non-renewable primary energy as energy carrier [MJ] 4.65E+0 2.94E-1 5.57E-2 0.00E+0 2.39E-1 -2.87E-1
Non-renewable primary energy as material utilization [MJ] 4.20E-2 0.00E+0 -4.20E-2 0.00E+0 0.00E+0 0.00E+0
Total use of non-renewable primary energy resources [MJ] 4.69E+0 2.94E-1 1.37E-2 0.00E+0 2.39E-1 -2.87E-1
Use of secondary material [kg] 0.00E+0 0.00E+0 0.00E+0 0.00E+0 0.00E+0 0.00E+0
Use of renewable secondary fuels [MJ] 0.00E+0 0.00E+0 0.00E+0 0.00E+0 0.00E+0 0.00E+0
Use of non-renewable secondary fuels [MJ] 0.00E+0 0.00E+0 0.00E+0 0.00E+0 0.00E+0 0.00E+0
Use of net fresh water [m³] 2.53E-2 2.29E-5 4.16E-4 0.00E+0 4.56E-5 -3.80E-5
RESULTS OF THE LCA – WASTE CATEGORIES AND OUTPUT FLOWS according to EN 15804+A1:
1 kg Reinforcement Fibre Plaster
Parameter Unit A1-A3 A4 A5 B1 C4 D
Hazardous waste disposed [kg] 1.65E-8 1.88E-8 1.31E-11 0.00E+0 4.12E-9 -1.61E-10
Non-hazardous waste disposed [kg] 7.05E-3 2.19E-5 1.97E-4 0.00E+0 1.12E+0 -1.55E-4
Radioactive waste disposed [kg] 1.20E-4 3.55E-7 5.52E-7 0.00E+0 3.43E-6 -1.26E-5
Components for re-use [kg] 0.00E+0 0.00E+0 0.00E+0 0.00E+0 0.00E+0 0.00E+0
Materials for recycling [kg] 0.00E+0 0.00E+0 1.25E-4 0.00E+0 0.00E+0 0.00E+0
Materials for energy recovery [kg] 0.00E+0 0.00E+0 2.59E-2 0.00E+0 0.00E+0 0.00E+0
Exported electrical energy [MJ] 0.00E+0 0.00E+0 5.96E-2 0.00E+0 0.00E+0 0.00E+0
Exported thermal energy [MJ] 0.00E+0 0.00E+0 1.40E-1 0.00E+0 0.00E+0 0.00E+0
6. LCA: Interpretation
The LCA results are dominated by the life cycle glass, dispersion powder, and hydrophobic agent
phases of raw material provision & transportation (A1 (together >80 % within A1). The manufacture of the
& A2), manufacture (particularly the manufacture of hydrophobic agent dominates the indicator ADPE
packaging in A3), and landfill disposal (C4) in all (approx. 80 %). The manufacture of the dispersion
impact categories. Taken together, approx. 80 – 95 % powder dominates the indicator ODP (>95 %).
of the environmental impact comes from these life Transportation of the raw materials plays a secondary
cycle phases. role (<10 % of total A1-A2).
In total, raw materials used and their transportation The manufacture of the packaging contributes (with the
contribute (excluding PERT and ODP) to the exception of GWP, ODP, and PERT) approx. 5 – 10 %.
environmental impact with a percentage of around 70 – The use of wooden pallets and paper contributes
90 % – primarily due to the use of cement, expanded significantly to PERT (approx. 50 % contribution).
Transportation of the products to the construction site In the usage phase, just over 20 % of the GWP caused
(A4) plays a secondary role (<10 %). is reabsorbed by means of carbonation (= carbon
dioxide absorption).
Landfill disposal at the end of the life cycle (C4)
contributes (excluding ADPE and ODP) approx. 0 – 10
% to the environmental impact.
7. Requisite evidence
7.1 Leaching: All specified products remained below the
All specified products in this LCA comply with all recommended limiting value.
emissions scenarios for a scenario involving the
building elements that are subject to moisture. 7.3 Radioactivity:
Measuring location: Fraunhofer Institute for Building
7.2 VOC emissions: Physics (IBP), Holzkirchen Branch, D-83626 Valley
Measuring location: Fraunhofer Institute for Building Measuring procedure: Test of content for the
Physics (IBP), Holzkirchen Branch, D-83626 Valley radioactive nuclides radium-226, thorium-232, and
Measuring procedure: Determination of volatile potassium-40 by measuring the activity concentrations
organic compounds from building products and fixtures CNuclide through alpha spectrometry (delayed
in accordance with DIN EN ISO 16000-9 and -11 in a coincidence method via LSC) or gamma spectrometry
0.2 m3 test chamber (t0 = 7 days) and evaluation as Test report: Inspection report from 12 December 2006
per the schema of the Committee for Health-related on the radioactivity of building products
Evaluation of Building Products (AgBB). Measurement Result: The activity concentration indices (I) calculated
of different products intended for both interior use and from the measured activity concentrations CNuclide
outdoors. were below the recommended limiting value of I = 2 for
Test report: Results log 005/2008/281 from 20 March all specified products. Moreover, at no point was the
2008 recommended limiting value I = 0.5 either reached or
Results: exceeded for building products used in large
quantities. Where I correlated with the dose criterion in
accordance with the Radiation Protection 112
guidelines from the European Commission, all
specified products remained below the recommended
limiting value of the annual radiation dose of 0.3
mSv/a.
8. References
PCR guidelines on building-related products and
services, Part A: Calculation rules for the Life Cycle GaBi 8
Assessment and requirements on the project report, GaBi 8.7 dataset documentation for the software-
Institut Bauen und Umwelt e. V., Version 1.7, 2018-03 system and databases, LBP, University of Stuttgart
and thinkstep, Leinfelden-Echterdingen, 2018
PCR guidelines on building-related products and (http://documentation.gabi-software.com/)
services, Part B: Requirements on the EPD for
mineral pre-made mortars, Institut Bauen und Umwelt
e. V., Version 1.6, 2017-11 DIN 4108-4
DIN 4108-4:2017-03, Thermal insulation and energy
IBU 2016 economy in buildings - Part 4: Hygrothermal design
IBU (2016): General EPD programme instructions from values
the
Institut Bauen und Umwelt e.V. (IBU). Version 1.1, DIN 18550-1
Institut Bauen und Umwelt e.V., Berlin. DIN 18550-1:2018-01, Design, preparation and
application of external rendering and internal
ISO 14025 plastering - Part 1: Supplementary provisions for
DIN EN ISO 14025:201110, DIN EN 13914-1:2016-09 for external rendering
Environmental labels and declarations - type III
environmental declarations - principles and DIN 18550-2
procedures. DIN 18550-2:2018-01, Design, preparation and
application of external rendering and internal
EN 15804 plastering - Part 2: Supplementary provisions for
EN 15804:201204+A1 2013, Sustainability of DIN EN 13914-2:2016-09 for internal plastering
construction works - Environmental product
declarations - DIN EN 197-1
Core rules for the product category of construction DIN EN 197-1:2011-11, Cement - Part 1: Composition,
products. specifications, and conformity criteria for common
9 Environmental Product Declaration Sto SE & Co. KGaA – Mineral pre-made mortar: rendering mortar – Reinforcement
Fibre Plaster
cements
DIN EN 16757
DIN EN 450-1 DIN EN 16757:2017-10, Sustainability of construction
DIN EN 450-1:2012-10, Fly ash for concrete - Part 1: works - Environmental product declarations - Product
Definition, specifications, and conformity criteria Category Rules for concrete and concrete elements
DIN EN 459-1 DIN EN ISO 14040
DIN EN 459-1:2015-07, Building lime - Part 1: DIN EN ISO 14040:2009-11, Environmental
Definitions, specifications, and conformity criteria management - Life cycle assessment - Principles and
framework (ISO 14040:2006)
DIN EN 998-1
DIN EN 998-1:2017-02, Specification for mortar for DIN EN ISO 14044
masonry - Part 1: Rendering and plastering mortar DIN EN ISO 14044:2018-05, Environmental
management - Life cycle assessment - Requirements
DIN EN 1015-10 and guidelines (ISO 14044:2006 + Amd 1:2017)
DIN EN 1015-10:2007-05, Methods of test for mortar
for masonry - Part 10: Determination of dry bulk DIN EN ISO 16000-9
density of hardened mortar DIN EN ISO 16000-9:2008-04, Indoor air - Part 9:
Determination of the emission of volatile organic
DIN EN 1015-11 compounds from building products and furnishing -
DIN EN 1015-11:2007-05, Methods of test for mortar Emission test chamber method
for masonry - Part 11: Determination of flexural and
compressive strength of hardened mortar DIN EN ISO 16000-11
DIN EN ISO 16000-11:2006-06, Indoor air - Part 11:
DIN EN 1015-18 Determination of the emission of volatile organic
DIN EN 1015-18:2003-03, Methods of test for mortar compounds from building products and furnishing -
for masonry - Part 18: Determination of water Sampling, storage of samples and preparation of test
absorption coefficient due to capillary action of specimens
hardened mortar
EC safety data sheet
DIN EN 1015-19 Available on the website of the relevant VDPM
DIN EN 1015-19:2005-01, Methods of test for mortar member company.
for masonry - Part 19: Determination of water vapour
permeability of hardened rendering and plastering ISO 15686-1
mortars ISO 15686-1:2011-05, Buildings and constructed
assets – Service life planning – Part 1: General
DIN EN 1052-3 principles and framework
DIN EN 1052-3:2007-06, Methods of test for masonry -
Part 3: Determination of initial shear strength ISO 15686-2
ISO 15686-2:2012-05, Buildings and constructed
DIN EN 1745 assets – Service life planning – Part 2: Service life
DIN EN 1745:2012-07 Masonry and masonry products prediction procedures
- Methods for determining thermal properties
ISO 15686-7
DIN EN 12664 ISO 15686-7:2017-04, Buildings and constructed
DIN EN 12664: 2001-05, Thermal performance of assets - Service life planning - Part 7: Performance
building materials and products - Determination of evaluation for feedback of service life data from
thermal resistance by means of guarded hot plate and practice
heat flow meter methods - Dry and moist products with
medium and low thermal resistance ISO 15686-8
ISO 15686-8:2008-06, Buildings and constructed
DIN EN 13501-1 assets - Service-life planning - Part 8: Reference
DIN EN 13501-1:2010-01, Fire classification of service life and service-life estimation
construction products and building elements - Part 1:
Classification using data from reaction to fire tests AgBB
Committee for Health-related Evaluation of Building
DIN EN 13914-1 Products (AgBB): Procedure for the health-related
DIN EN 13914-1:2016-09, Design, preparation and evaluation of volatile organic compound (VOC)
application of external rendering and internal plastering emissions from building products
- Part 1: External rendering
AVV
DIN EN 13914-2 Waste Catalogue Ordinance dated 10 December 2001
DIN EN 13914-2:2016-09, Design, preparation and (Federal Law Gazette I p. 3379), last amended by
application of external rendering and internal plastering Article 2 of the Regulation of 17 July 2017 (Federal
- Part 2: Internal plastering Law Gazette I. p. 2644)
DIN EN 13914-2 Corrigendum 1 BBSR
DIN EN 13914-2 Corrigendum 1:2017-05, Design, BBSR - Federal Office for Building and Regional
preparation and application of external rendering and Planning: Nutzungsdauern von Bauteilen für
internal plastering - Part 2: Internal plastering; Lebenszyklusanalysen nach Bewertungssystem
Corrigendum to DIN EN 13914-2:2016-09 Nachhaltiges Bauen (BNB) (Service lives of building
10 Environmental Product Declaration Sto SE & Co. KGaA – Mineral pre-made mortar: rendering mortar – Reinforcement
Fibre Plaster
elements for Life Cycle Assessments conducted Commission Decision of 9 September 1994
according to the BNB Sustainable Building assessment implementing Article 20 of Directive 89/106/EEC on
system), dated 24 February 2017 construction products (94/611/EC)
German Building Materials Association Life Cycle Assessment
Bundesverband Baustoffe – Steine und Erden Comparative Life Cycle Assessment: Masonry with
(German Building Materials Association) (Ed.): mineral mortar and masonry with PU foam bonding in
Mineralische Bauabfälle – Monitoring 2010 (Mineral accordance with ISO 14040 and ISO 14044; carried
construction waste – monitoring 2010); Berlin, 2013 out on behalf of the VDPM (formerly IWM); Fraunhofer
Institute for Building Physics IBP, Stuttgart/Holzkirchen
DepV (2009) 2008
Ordinance on Landfills and Long-Term Storage
Facilities – Landfill Ordinance of 27 April 2009 (Federal Radiation Protection 112
Law Gazette I p. 900); last modified by Article 2 of the European Commission: Radiation Protection 112
Regulation of 27 September 2017 (Federal Law “Radiological protection principles concerning the
Gazette I p. 3465). natural radioactivity of building materials”,
Luxembourg: Publications Office of the European
ECHA candidate list Union, 2000
European Chemicals Agency (ECHA): List of
Substances of Very High Concern (published in SAF
accordance with Article 59 Para. 10 of the REACH SAF – Fachverband der Stuckateure für Ausbau und
Regulation) Fassade Baden-Württemberg e.V. (Association of
Plasterers for Finishing and Facade) (Ed.): “Facade
EWC waste code base render / outside facilities” guidelines, 3rd edition
Ordinance regarding the introduction of the European 2013
Waste Catalogue (EWC Ordinance) from 13
September 1996: six-figure designation of types of TASi
waste, provided movable objects are waste according Technical Guidelines for the Recovery, Treatment and
to Art. 3 Para. 1 of the Closed Substance Cycle and Other Forms of Management of Domestic Waste (Third
Waste Management Act General Administrative Regulation for the Waste Act)
from 14 May 1993 (Federal Gazette No. 99a of 29 May
Industrieverband Werktrockenmörtel e.V. (WTM) 1993)
Internal study “Ökologische Aspekte von
Werktrockenmörtel” (Ecological aspects of ready
mixed dry render), January 2000 edition (unpublished)
Commission Decision 94/611/EC
11 Environmental Product Declaration Sto SE & Co. KGaA – Mineral pre-made mortar: rendering mortar – Reinforcement
Fibre Plaster
Publisher
Institut Bauen und Umwelt e.V. Tel +49 (0)30 3087748- 0
Panoramastr. 1 Fax +49 (0)30 3087748- 29
10178 Berlin Mail info@ibu-epd.com
Germany Web www.ibu-epd.com
Programme holder
Institut Bauen und Umwelt e.V. Tel +49 (0)30 - 3087748- 0
Panoramastr 1 Fax +49 (0)30 – 3087748 - 29
10178 Berlin Mail info@ibu-epd.com
Germany Web www.ibu-epd.com
Author of the Life Cycle
Assessment Tel +49 (0) 711 341817-0
thinkstep AG Fax +49(0) 711 341817-25
Hauptstrasse 111-113 Mail info@thinkstep.com
D-70771 Leinfelden-Echterdingen Web http://www.thinkstep.com
Germany
Owner of the Declaration
Sto SE & Co. KGaA Tel +49 7744 57-1010
Ehrenbachstr. 1 Fax +49 7744 57-2010
79780 Stühlingen Mail infoservice@sto.com
Germany Web www.sto.com
