Environmental Product Declaration (EPD)
According to ISO 14025 and EN 15804
StoLevell Evo
Registration number: EPD-Kiwa-EE-162142-EN
Issue date: 20-12-2023
Valid until: 20-12-2028
Declaration owner: Sto SE & Co. KGaA
Publisher: Kiwa-Ecobility Experts
Program operator: Kiwa-Ecobility Experts
Status: verified
StoLevell Evo | ReTHiNK-62142 1 / 19
Environmental Product Declaration
1 General information
E-mail: infoservice@sto.com
1.1 PRODUCT Website: https://www.sto.com
Production location: Sto Scandinavia AB
StoLevell Evo
Address production location: Gesällgatan 6, 582 77 Linköping, Sweden
1.2 REGISTRATION NUMBER
1.6 VERIFICATION OF THE DECLARATION
EPD-Kiwa-EE-162142-EN
The independent verification is in accordance with the ISO 14025:2011. The LCA is in
1.3 VALIDITY compliance with ISO 14040:2006 and ISO 14044:2006. The EN 15804:2012+A2:2019 serves as
the core PCR.
Issue date: 20-12-2023
Internal ✓ External
Valid until: 20-12-2028
1.4 PROGRAM OPERATOR
Kiwa-Ecobility Experts
Voltastraße 5
13355 Berlin
DE
Lucas Pedro Berman, Senda
1.7 STATEMENTS
Prof. Dr. Frank Heimbecher
The owner of this EPD shall be liable for the underlying information and evidence. The
(Chairman of the independent expert
programme operator Kiwa-Ecobility Experts shall not be liable with respect to
committee - Kiwa-Ecobility Experts)
manufacturer data, life cycle assessment data and evidence.
Frank Huppertz 1.8 PRODUCT CATEGORY RULES
(Head of Kiwa-Ecobility Experts)
Kiwa-Ecobility Experts (Kiwa-EE) – General Product Category Rules (2022-02-14)
Institut Bauen und Umwelt e.V - Complementary Product Category Rule (c-PCR):
1.5 OWNER OF THE DECLARATION
Requirements on the EPD for Mineral factory-made mortar - 12/07/2023 v3
Manufacturer: Sto SE & Co. KGaA
Address: Ehrenbachstraße 1, D-79780 Stühlingen
StoLevell Evo | ReTHiNK-62142 2 / 19
Environmental Product Declaration
1 General information
1.9 COMPARABILITY 1.10 CALCULATION BASIS
In principle, a comparison or assessment of the environmental impacts of different LCA method R<THiNK: Ecobility Experts | EN15804+A2
products is only possible if they have been prepared in accordance with EN 15804. For the
evaluation of the comparability, the following aspects have to be considered in particular: LCA software*: Simapro 9.1
PCR used, functional or declared unit, geographical reference, the definition of the system Characterization method: EN 15804 +A2 Method v1.0
boundary, declared modules, data selection (primary or secondary data, background
database, data quality), scenarios used for use and disposal phases, and the life cycle LCA database profiles: EcoInvent version 3.6
inventory (data collection, calculation methods, allocations, validity period). PCRs and Version database: v3.15 (2023-07-12)
general program instructions of different EPDs programs may differ. Comparability needs
to be evaluated. For further guidance, see EN 15804+A2 (5.3 Comparability of EPD for * Used for calculating the characterized results of the Environmental profiles within
construction products) and ISO 14025 (6.7.2 Requirements for comparability). R<THiNK.
1.11 LCA BACKGROUND REPORT
This EPD is generated on the basis of the LCA background report 'StoLevell Evo' with the
calculation identifier ReTHiNK-62142.
StoLevell Evo | ReTHiNK-62142 3 / 19
Environmental Product Declaration
2 Product
2.1 PRODUCT DESCRIPTION
Pour the water and add the dry mortar. Mix well and let it rest for approx. 5 minutes before
use.
StoLevell Evo is a pumpable cementitious mortar designed as a base coat for mineral
substrates, EPS and mineral wool boards. It can be applied as plastering mortar on walls,
2.3 REFERENCE SERVICE LIFE
ceilings, pillars and separating walls, both indoors and outdoors. StoLevell Evo is also used
as a base coat in several of Sto’s facade systems.
RSL PRODUCT
StoLevell Evo is supplied in 25 kg small bags (paper/polyethylene plastic (PE)) or in 1000 kg A reference service life (RSL) as per ISO 15686-1, -2, - 7, and -8 is not declared. Provided they
big bags (polypropylene- and polyethylene plastic (PP/LDPE)). are used as intended and properly applied, the service life of rendering and plastering
mortars made from mineral pre-made mortars on walls and ceilings has been known to
StoLevell Evo is compliant with EN 998-1:2016 General purpose plastering mortar (GP) CS
be 40 years or longer (according to BBSR - The Federal Office for Building and Regional
III.
Planning). In this life cycle analysis the RSL of 50 years has been declared, equal to the
useful life of the building (according to standard 15804:A2).
USED RSL (YR) IN THIS LCA CALCULATION:
50
2.4 TECHNICAL DATA
Density, dry powder: 1,200 kg/cm³
Density, hardened: 1,600 kg/cm³
Characteristics
• good adhesion
2.2 APPLICATION (INTENDED USE OF THE PRODUCT)
• weather-resistant
• highly water-repellent
StoLevell Evo is a pre-made cementitious dry mortar that is polymer modified. Pre-made • high water transmission
dry mortar is a mortar made from raw materials that are placed into containers dry at the
factory, delivered to the construction site, and then mixed with the required quantity of
water to form ready-to-use mortar based on the manufacturer’s instructions and 2.5 SUBSTANCES OF VERY HIGH CONCERN
conditions.
The product does not contain substances of very high concern (SVHC) on the REACH
Application temperature
Candidate List published by the European Chemicals Agency in a concentration more
than 0,1 % (by unit weight).
Lowest substrate and air temperature: +5 °C
The product is categorized as non-hazardous waste with code 17 01 01 (hardened mortar).
Highest substrate and air temperature: +30 °C
Mixing ratio
2.6 DESCRIPTION PRODUCTION PROCESS
4.75 L of water per 25 kg
StoLevell Evo is produced in Linköping, Sweden, by Sto Scandinavia AB. Sto Scandinavia
Material preparation AB is a subsidiary of Sto SE & Co. KGaA. The raw materials that are used in StoLevell Evo are
StoLevell Evo | ReTHiNK-62142 4 / 19
Environmental Product Declaration
2 Product
produced and transported from suppliers located in Europe. Main market is the Nordic
countries.
The production process starts from raw materials that are purchased from external
suppliers and transported to the manufacturing plant in Linköping. The raw materials are
then stored at the plant in silos, gravimetrically dosed and intensely mixed in the
production mixer according to the formula of the product. The production is a
discontinuous process, in which all the components are mechanically mixed in batches.
The mixed and finished product is then packaged in paper/PE bags or in big bags of PP/
LDPE, put on wooden pallets, covered with wrapping material (stretch film) and stored in
the production warehouse. The quality of the final product is controlled before the sale.
The energy that is used during production is electricity and also heat for warming up the
factory. Emissions during production consist of indoor dust in the factory. There is no
release of dust to the outdoor environment. Waste during production is less than 1% (0.14%
according to production figures). Waste is in the form of cementitious dust from the
mixing process.
Product Flow Diagram
This diagram shows the different life cycle stages of StoLevell Evo. The stages concerning
the production process is shown under A3.
2.7 CONSTRUCTION DESCRIPTION
StoLevell Evo is a dry cementitious mortar that is mixed with water at the construction site
before application. The mixed mortar is applied in layers of 6-15 mm and applied
mechanically with a plaster gun or manually by hand. Surface treatment is then done with
a trowel or a plasterer's float.
The drying time depends on the temperature, wind and relative air humidity. Appropriate
measures need to be taken to protect ongoing or newly plastered external walls in bad
weather (e.g. apply a rain cover). Hardening takes approx. 1 day per mm of layer thickness,
depending on weather conditions.
At an air and substrate temperature of +20 °C and 65% relative air humidity, the layer is
over-coatable after approx. 24 hours.
StoLevell Evo | ReTHiNK-62142 5 / 19
Environmental Product Declaration
3 Calculation rules
3.1 DECLARED UNIT Module A5 = Construction -
Module C2 = Transport
Installation process
1 kg
Module B1 = Use Module C3 = Waste Processing
Declared unit is 1 kg of StoLevell Evo installed and with an RSL of 50 years. The product is in
Module B2 = Maintenance Module C4 = Disposal
dry state according to PCR for Mineral factory-made mortar. StoLevell Evo is a pre-made
cementitious dry mortar. Module D = Benefits and loads beyond the
Module B3 = Repair
product system boundaries
The scope of this LCA is cradle to gate with options, modules C1-C4 and module D.
Technical life span of the products raw materials is the same as for the whole product. Module B4 = Replacement
Reference Service Life of the product is the same as estimated lifetime of the building in
which the product is being used.
3.4 REPRESENTATIVENESS
reference_unit: kilogram (kg)
The input data are representative for StoLevell Evo, a product of Sto SE & Co. KGaA. The
data are representative for the European Union.
3.2 CONVERSION FACTORS
The scenarios included in this life cycle analysis are currently in use and are representative
for one of the most likely scenario alternatives.
Description Value Unit
reference_unit 1 kg
3.5 CUT-OFF CRITERIA
Conversion factor to 1 kg 1.000000 kg
Criteria for the exclusion of inputs and outputs (cut-off rules) in the LCA, information
modules and any additional information are intended to support an efficient calculation
3.3 SCOPE OF DECLARATION AND SYSTEM BOUNDARIES procedure. They are not applied in order to hide data.
This is a Cradle to gate with options, modules C1-C4 and module D LCA. The life cycle
Product Stage (A1-A3)
stages included are as shown below:
(X = module included, ND = module not declared) The production stage consists of the extraction of raw materials, transportation of the raw
materials, processing the raw materials into materials and the production of the product.
A1 A2 A3 A4 A5 B1 B2 B3 B4 B5 B6 B7 C1 C2 C3 C4 D
The required energy for production, ancillary materials, packaging materials and
X X X X X ND ND ND ND ND ND ND X X X X X production emissions are included.
All substantial raw materials and types of energy during production are included. Raw
materials added to the product in very small amounts (less than 1%) are not included.
The modules of the EN15804 contain the following:
These cut-off limits do not apply to hazardous materials or substances.
Module A1 = Raw material supply Module B5 = Refurbishment
As StoLevell Evo is a mortar, there are no co-products that have to be taken into account.
Module A2 = Transport Module B6 = Operational energy use
Module A3 = Manufacturing Module B7 = Operational water use Construction process stage (A4-A5)
Module A4 = Transport Module C1 = De-construction / Demolition
This stage consists of the transportation of the product from production plant to the
construction site.
StoLevell Evo | ReTHiNK-62142 6 / 19
Environmental Product Declaration
3 Calculation rules
It also includes the loss of material during construction. The additional needed production,
transport and end-of-life of the lost material during construction is included. 3.6 ALLOCATION
The end-of-life of packaging material up to the end-of-waste state or disposal of final The amount of electricity at the production site for StoLevell Evo comes from figures
residues is also included. concerning the total amount of electricity being used at the site (for all products
produced) and then recalculated into the amount only used for producing StoLevell Evo at
the site. The amount of electricity is then shown per kg produced product.
End of life stage (C1-C4)
The amount of energy used for heating at the production site for StoLevell Evo comes
When the end of the life stage of the building is reached, the de-construction/demolition
from figures concerning the total amount of district heating used at the site (for all
begins. This EPD includes de-construction/demolition (C1), the necessary transport (C2)
products produced) and then recalculated into the amount only used to produce StoLevell
from the demolition site to the sorting location and distance to final disposal. The end of
Evo at the site. The amount of district heating is then shown per kg produced product.
life stage includes the final disposal to landfill (C4), incineration (C3) and needed recycling
processes up to the end-of-waste point (C3). Loads and benefits of recycling, re-use and Modularity principle has been taken into account. Since StoLevell Evo is a mortar, there are
exported energy are part of module D. no co-products that have to be taken into account.
The prescribed waste scenarios from the NMD Determination Method V1.1 have been used The producer of StoLevell Evo is under regulation from national authorities and follows the
for the various materials in the product. polluter pays principle.
Benefits and Loads beyond the system boundary (Module D) 3.7 DATA COLLECTION & REFERENCE TIME PERIOD
This stage contains the potential loads and benefits of recycling and re-use of raw
This EPD project has been performed during the year 2023. Production data is for the year
materials/products. The loads contain the needed recycling processes from end-of-waste-
2022.
point up to the point-of-equivalence of the substituted primary raw material and a load for
secondary material that will be lost at the end-of-life stage.
3.8 ESTIMATES AND ASSUMPTIONS
The loads and benefits of recycling and reuse are included in this module. The benefits are
calculated based on the primary content and the primary equivalent.
Mortar is categorized as mineral construction waste. The European Waste Code (EWC) for
In addition, the benefits of energy recovery are granted at this stage. The amount of avoid mortar is 17 01 01 (Concrete from construction and demolition activities) and is categorized
energy is based on the Lower Heating Values of the materials and the efficiencies of the as non-hazardous waste. Mortar can therefore be used in landfills. This code applies for
incinerators as mentioned in the NMD Determination Method V1.1 or EcoInvent 3.6 (2019). hardened mortar.
The end of life scenario reflects the Nordic market, where 87% of mineral waste from
construction and demolition is estimated to be landfilled and 13% is recycled (8).
Excluded processes
Following processes has not been taken into account in this life cycle analysis: 3.9 DATA QUALITY
• The manufacture of equipment used in production, buildings or any other capital
Specific data on the product's constituent raw materials have been collected during the
goods;
year 2023. Raw material suppliers have been contacted to obtain an EPD for each raw
• The transportation of personnel to the production plant;
material. In cases where suppliers did not have EPDs according to EN 15804, data from
• The transportation of personnel within the production plant;
LCA database EcoInvent 3.6 were used.
• Research and development activities;
• Long-term emissions.
StoLevell Evo | ReTHiNK-62142 7 / 19
Environmental Product Declaration
3 Calculation rules
Data concerning production has been collected from the Production Management
System used at the production site and the figures shown in this report is for the year 3.10 GUARANTEES OF ORIGIN
2022.
Local based approach has been applied. Therefore the Swedish consumption mix (=
national production + imports - exports) was used to consider the impact of electricity. No
GOs need to be specified when using this method.
StoLevell Evo | ReTHiNK-62142 8 / 19
Environmental Product Declaration
4 Scenarios and additional technical information
4.1 TRANSPORT TO CONSTRUCTION SITE (A4)
For the transport from production place to assembly/user, the following scenario is
assumed for module A4 of this EPD.
Value and unit
Vehicle type used for transport Lorry (Truck) 16-32t, EURO6 | market for (EU)
Fuel type and consumption of vehicle not available
Distance 200 km
Capacity utilisation (including empty returns) 50 % (loaded up and return empty)
Bulk density of transported products inapplicable
Volume capacity utilisation factor 1
4.2 ASSEMBLY (A5)
The following information describes the scenarios for flows entering the system and flows
leaving the system at module A5.
FLOWS ENTERING THE SYSTEM
For flows entering the system at A5 the following scenario is assumed for module A5.
Value Unit
Materials used for installation/assembly
Surface water 0.2 kg
Energy consumption for installation/assembly
Electricity (SE) - low voltage (max 1kV) 0.0027 kWh
FLOWS LEAVING THE SYSTEM
The following output flows leaving the system at module A5 are assumed.
Description Value Unit
Output materials as result of loss during construction 3 %
Output materials as result of waste processing of materials used for installation/assembly at the building site 0.000 kg
Output materials as result of waste processing of used packaging 0.021 kg
StoLevell Evo | ReTHiNK-62142 9 / 19
Environmental Product Declaration
4 Scenarios and additional technical information
4.3 DE-CONSTRUCTION, DEMOLITION (C1)
No inputs are needed for the product at the de-construction / demolition phase
4.4 TRANSPORT END-OF-LIFE (C2)
The following distances and transport conveyance are assumed for transportation during
end of life for the different types of waste processing.
Waste Scenario Transport conveyance Not removed (stays in work) [km] Landfill [km] Incineration [km] Recycling [km] Re-use [km]
Debris - STO Sweden Lorry (Truck), unspecified (default) | market group for (GLO) 0 100 150 50 0
The transport conveyance(s) used in the scenario(s) for transport during end of life has the
following characteristics.
Value and unit
Vehicle type used for transport Lorry (Truck), unspecified (default) | market group for (GLO)
Fuel type and consumption of vehicle not available
Capacity utilisation (including empty returns) 50 % (loaded up and return empty)
Bulk density of transported products inapplicable
Volume capacity utilisation factor 1
4.5 END OF LIFE (C3, C4)
The scenario(s) assumed for end of life of the product are given in the following tables.
First the assumed percentages per type of waste processing are displayed, followed by the
assumed amounts.
Waste Scenario Region Not removed (stays in work) [%] Landfill [%] Incineration [%] Recycling [%] Re-use [%]
Debris - STO Sweden NL 0 87 0 13 0
Waste Scenario Not removed (stays in work) [kg] Landfill [kg] Incineration [kg] Recycling [kg] Re-use [kg]
Debris - STO Sweden 0.000 0.870 0.000 0.130 0.000
Total 0.000 0.870 0.000 0.130 0.000
StoLevell Evo | ReTHiNK-62142 10 / 19
Environmental Product Declaration
4 Scenarios and additional technical information
4.6 BENEFITS AND LOADS BEYOND THE SYSTEM BOUNDARY (D)
The presented Benefits and loads beyond the system boundary in this EPD are based on
the following calculated Net output flows in kilograms and Energy recovery displayed in
MJ Lower Heating Value.
Waste Scenario Net output flow [kg] Energy recovery [MJ]
Debris - STO Sweden 0.130 0.000
Total 0.130 0.000
StoLevell Evo | ReTHiNK-62142 11 / 19
Environmental Product Declaration
5 Results
For the impact assessment, the characterization factors of the LCIA method EN 15804 +A2
Method v1.0 are used. Long-term emissions (>100 years) are not considered in the impact
assessment. The results of the impact assessment are only relative statements that do not
make any statements about end-points of the impact categories, exceedance of threshold
values, safety margins or risks. The following tables show the results of the indicators of the
impact assessment, of the use of resources as well as of waste and other output flows.
5.1 ENVIRONMENTAL IMPACT INDICATORS PER KILOGRAM
CORE ENVIRONMENTAL IMPACT INDICATORS EN15804+A2
Abbreviation Unit A1 A2 A3 A4 A5 C1 C2 C3 C4 D
AP mol H+ eqv. 4.78E-4 8.66E-5 9.61E-5 9.61E-5 3.58E-5 0.00E+0 7.32E-5 1.33E-6 4.35E-5 -3.85E-5
GWP-total kg CO2 eqv. 1.62E-1 2.69E-2 -1.24E-2 3.35E-2 4.34E-2 0.00E+0 1.26E-2 2.13E-4 4.59E-3 -2.57E-3
GWP-b kg CO2 eqv. 1.68E-4 2.04E-5 -2.97E-2 1.80E-5 3.36E-2 0.00E+0 5.83E-6 1.22E-6 9.08E-6 -1.09E-4
GWP-f kg CO2 eqv. 1.62E-1 2.69E-2 1.73E-2 3.34E-2 9.75E-3 0.00E+0 1.26E-2 2.11E-4 4.58E-3 -2.44E-3
GWP-luluc kg CO2 eqv. 4.49E-5 8.20E-6 6.87E-5 1.19E-5 1.34E-5 0.00E+0 4.62E-6 4.02E-8 1.28E-6 -1.27E-5
EP-m kg N eqv. 9.62E-5 1.90E-5 2.43E-5 1.90E-5 9.80E-6 0.00E+0 2.58E-5 5.28E-7 1.50E-5 -1.12E-5
EP-fw kg P eqv. 3.08E-6 2.14E-7 8.98E-7 2.67E-7 1.61E-7 0.00E+0 1.27E-7 6.59E-9 5.14E-8 -1.31E-7
EP-T mol N eqv. 9.67E-4 2.12E-4 2.71E-4 2.13E-4 1.06E-4 0.00E+0 2.84E-4 5.87E-6 1.65E-4 -1.77E-4
kg CFC 11
ODP 4.79E-9 6.61E-9 1.85E-9 7.61E-9 9.89E-10 0.00E+0 2.79E-9 2.74E-11 1.89E-9 -4.64E-10
eqv.
kg NMVOC
POCP 3.37E-4 8.31E-5 9.70E-5 8.15E-5 3.33E-5 0.00E+0 8.12E-5 1.59E-6 4.79E-5 -3.30E-5
eqv.
ADP-f MJ 1.85E+0 4.37E-1 3.05E-1 5.06E-1 1.28E-1 0.00E+0 1.90E-1 2.84E-3 1.28E-1 -3.44E-2
ADP-mm kg Sb-eqv. 9.25E-7 4.79E-7 2.72E-7 9.23E-7 1.07E-7 0.00E+0 3.20E-7 5.97E-10 4.19E-8 -4.47E-8
m3 world
WDP 1.51E+0 1.42E-3 1.31E-2 1.43E-3 4.64E-2 0.00E+0 6.81E-4 1.29E-5 5.74E-3 -8.27E-3
eqv.
AP=Acidification (AP) | GWP-total=Global warming potential (GWP-total) | GWP-b=Global warming potential - Biogenic (GWP-b) | GWP-f=Global warming potential - Fossil (GWP-f) | GWP-
luluc=Global warming potential - Land use and land use change (GWP-luluc) | EP-m=Eutrophication marine (EP-m) | EP-fw=Eutrophication, freshwater (EP-fw) | EP-T=Eutrophication,
terrestrial (EP-T) | ODP=Ozone depletion (ODP) | POCP=Photochemical ozone formation - human health (POCP) | ADP-f=Resource use, fossils (ADP-f) | ADP-mm=Resource use, minerals and
metals (ADP-mm) | WDP=Water use (WDP)
StoLevell Evo | ReTHiNK-62142 12 / 19
Environmental Product Declaration
5 Results
ADDITIONAL ENVIRONMENTAL IMPACT INDICATORS EN15084+A2
Abbreviation Unit A1 A2 A3 A4 A5 C1 C2 C3 C4 D
ETP-fw CTUe 1.01E+0 3.48E-1 6.17E-1 4.07E-1 1.14E-1 0.00E+0 1.70E-1 2.30E-3 8.31E-2 -3.37E-1
disease
PM 3.87E-9 2.36E-9 1.10E-7 2.13E-9 3.70E-9 0.00E+0 1.14E-9 2.93E-11 8.45E-10 -5.37E-10
incidence
HTP-c CTUh 2.35E-11 8.44E-12 2.99E-11 1.13E-11 8.27E-12 0.00E+0 5.50E-12 5.46E-14 1.92E-12 -4.23E-12
HTP-nc CTUh 7.50E-10 3.81E-10 3.47E-10 4.29E-10 9.85E-11 0.00E+0 1.86E-10 1.54E-12 5.90E-11 -1.49E-10
IR kBq U235 eqv. 2.31E-3 1.91E-3 1.23E-3 2.21E-3 8.56E-4 0.00E+0 7.97E-4 9.00E-6 5.25E-4 -9.04E-5
SQP Pt 9.95E-1 5.00E-1 5.59E+0 3.54E-1 2.51E-1 0.00E+0 1.65E-1 4.74E-4 2.69E-1 -1.34E+0
ETP-fw=Ecotoxicity, freshwater (ETP-fw) | PM=Particulate Matter (PM) | HTP-c=Human toxicity, cancer (HTP-c) | HTP-nc=Human toxicity, non-cancer (HTP-nc) | IR=Ionising radiation, human
health (IR) | SQP=Land use (SQP)
CLASSIFICATION OF DISCLAIMERS TO THE DECLARATION OF CORE AND ADDITIONAL ENVIRONMENTAL IMPACT INDICATORS
ILCD classification Indicator Disclaimer
Global warming potential (GWP) None
ILCD type / level 1 Depletion potential of the stratospheric ozone layer (ODP) None
Potential incidence of disease due to PM emissions (PM) None
AAcidification potential, Accumulated Exceedance (AP) None
Eutrophication potential, Fraction of nutrients reaching freshwater end compartment
None
(EP-freshwater)
Eutrophication potential, Fraction of nutrients reaching marine end compartment
ILCD type / level 2 None
(EP-marine)
Eutrophication potential, Accumulated Exceedance (EP-terrestrial) None
Formation potential of tropospheric ozone (POCP) None
Potential Human exposure efficiency relative to U235 (IRP) 1
Abiotic depletion potential for non-fossil resources (ADP-minerals&metals) 2
ILCD type / level 3
Abiotic depletion potential for fossil resources (ADP-fossil) 2
Water (user) deprivation potential, deprivation-weighted water consumption (WDP) 2
Potential Comparative Toxic Unit for ecosystems (ETP-fw) 2
StoLevell Evo | ReTHiNK-62142 13 / 19
Environmental Product Declaration
5 Results
ILCD classification Indicator Disclaimer
Potential Comparative Toxic Unit for humans (HTP-c) 2
Potential Comparative Toxic Unit for humans (HTP-nc) 2
Potential Soil quality index (SQP) 2
Disclaimer 1 – This impact category deals mainly with the eventual impact of low dose ionizing radiation on human health of the nuclear fuel cycle. It does not consider effects due to possible
nuclear accidents, occupational exposure nor due to radioactive waste disposal in underground facilities. Potential ionizing radiation from the soil, from radon and from some construction
materials is also not measured by this indicator.
Disclaimer 2 – The results of this environmental impact indicator shall be used with care as the uncertainties on these results are high or as there is limited experienced with the indicator.
5.2 INDICATORS DESCRIBING RESOURCE USE AND ENVIRONMENTAL INFORMATION BASED ON LIFE CYCLE INVENTORY (LCI)
PARAMETERS DESCRIBING RESOURCE USE
Abbreviation Unit A1 A2 A3 A4 A5 C1 C2 C3 C4 D
PERE MJ 1.02E-1 5.50E-3 5.54E-1 7.24E-3 2.82E-2 0.00E+0 2.38E-3 1.62E-4 1.04E-3 -2.75E-1
PERM MJ 0.00E+0 0.00E+0 2.80E-1 0.00E+0 8.39E-3 0.00E+0 0.00E+0 0.00E+0 0.00E+0 0.00E+0
PERT MJ 1.02E-1 5.50E-3 8.34E-1 7.24E-3 3.66E-2 0.00E+0 2.38E-3 1.62E-4 1.04E-3 -2.75E-1
PENRE MJ 1.35E+0 4.64E-1 3.03E-1 5.37E-1 1.16E-1 0.00E+0 2.02E-1 3.03E-3 1.36E-1 -3.63E-2
PENRM MJ 6.16E-1 0.00E+0 2.17E-2 0.00E+0 1.91E-2 0.00E+0 0.00E+0 0.00E+0 0.00E+0 -8.21E-4
PENRT MJ 1.97E+0 4.64E-1 3.25E-1 5.37E-1 1.35E-1 0.00E+0 2.02E-1 3.03E-3 1.36E-1 -3.71E-2
SM Kg 9.36E-4 0.00E+0 1.31E-6 0.00E+0 2.81E-5 0.00E+0 0.00E+0 0.00E+0 0.00E+0 0.00E+0
RSF MJ 3.61E-2 0.00E+0 5.06E-5 0.00E+0 1.09E-3 0.00E+0 0.00E+0 0.00E+0 0.00E+0 0.00E+0
NRSF MJ 4.04E-1 0.00E+0 5.66E-4 0.00E+0 1.21E-2 0.00E+0 0.00E+0 0.00E+0 0.00E+0 0.00E+0
FW M3 1.81E-3 4.97E-5 2.98E-4 5.41E-5 1.01E-4 0.00E+0 2.32E-5 9.49E-7 1.37E-4 -1.94E-4
PERE=renewable primary energy ex. raw materials | PERM=renewable primary energy used as raw materials | PERT=renewable primary energy total | PENRE=non-renewable primary energy
ex. raw materials | PENRM=non-renewable primary energy used as raw materials | PENRT=non-renewable primary energy total | SM=use of secondary material | RSF=use of renewable
secondary fuels | NRSF=use of non-renewable secondary fuels | FW=use of net fresh water
StoLevell Evo | ReTHiNK-62142 14 / 19
Environmental Product Declaration
5 Results
OTHER ENVIRONMENTAL INFORMATION DESCRIBING WASTE CATEGORIES
Abbreviation Unit A1 A2 A3 A4 A5 C1 C2 C3 C4 D
HWD Kg 1.70E-5 1.06E-6 5.66E-6 1.32E-6 7.96E-7 0.00E+0 4.82E-7 4.95E-9 1.91E-7 -7.70E-8
NHWD Kg 9.84E-3 3.80E-2 5.87E-3 2.46E-2 3.15E-2 0.00E+0 1.21E-2 3.96E-4 8.70E-1 -5.76E-4
RWD Kg 6.73E-6 2.98E-6 1.55E-6 3.44E-6 7.98E-7 0.00E+0 1.25E-6 1.28E-8 8.41E-7 -1.22E-7
HWD=hazardous waste disposed | NHWD=non hazardous waste disposed | RWD=radioactive waste disposed
ENVIRONMENTAL INFORMATION DESCRIBING OUTPUT FLOWS
Abbreviation Unit A1 A2 A3 A4 A5 C1 C2 C3 C4 D
CRU Kg 0.00E+0 0.00E+0 0.00E+0 0.00E+0 0.00E+0 0.00E+0 0.00E+0 0.00E+0 0.00E+0 0.00E+0
MFR Kg 1.92E-5 0.00E+0 2.69E-8 0.00E+0 4.96E-3 0.00E+0 0.00E+0 1.30E-1 0.00E+0 0.00E+0
MER Kg 8.07E-5 0.00E+0 1.13E-7 0.00E+0 2.43E-6 0.00E+0 0.00E+0 0.00E+0 0.00E+0 0.00E+0
EET MJ 1.18E-4 0.00E+0 1.65E-7 0.00E+0 3.55E-6 0.00E+0 0.00E+0 0.00E+0 0.00E+0 8.16E-2
EEE MJ 7.81E-6 0.00E+0 1.09E-8 0.00E+0 2.35E-7 0.00E+0 0.00E+0 0.00E+0 0.00E+0 4.74E-2
CRU=Components for re-use | MFR=Materials for recycling | MER=Materials for energy recovery | EET=Exported Energy Thermic | EEE=Exported Energy Electric
StoLevell Evo | ReTHiNK-62142 15 / 19
Environmental Product Declaration
5 Results
5.3 INFORMATION ON BIOGENIC CARBON CONTENT PER KILOGRAM
BIOGENIC CARBON CONTENT
The following Information describes the biogenic carbon content in (the main parts of) the
product at the factory gate per kilogram:
Biogenic carbon content Amount Unit
Biogenic carbon content in the product 0 kg C
Biogenic carbon content in accompanying packaging 0.009091 kg C
UPTAKE OF BIOGENIC CARBON DIOXIDE
The following amount of uptake of carbon dioxide is account in module A1 by the main
parts of the product. Related uptake and release of carbon dioxide in downstream
processes are not taken into account in this number although they do appear in the
presented results.
Uptake Biogenic Carbon dioxide Amount Unit
Packaging 0.03333 kg CO2 (biogenic)
StoLevell Evo | ReTHiNK-62142 16 / 19
Environmental Product Declaration
6 Interpretation of results
The figure above shows the influence of the different life stages on the LCA results. The raw
materials for StoLevell Evo (A1) contribute the most to the total GWP values, followed by
the installation and use of the product at the construction site (A5). The main
environmental impacts of the product's life cycle come from the product stage A1-A3. The
extraction of raw materials (A1) has the largest impact (especially for water resource
utilization, GWP-fossil and eutrophication in fresh water), followed by the manufacturing
stage (A3) and lastly the transportation of raw materials to the manufacturing site (A2).
StoLevell Evo | ReTHiNK-62142 17 / 19
Environmental Product Declaration
7 References
1. ISO 14040
ISO 14040:2006-10, Environmental management - Life cycle assessment - Principles and framework; EN ISO 14040:2006
2. ISO 14044
ISO 14044:2006-10, Environmental management - Life cycle assessment - Requirements and guidelines; EN ISO 14040:2006
3. ISO 14025
ISO 14025:2011-10: Environmental labels and declarations — Type III environmental declarations — Principles and procedures
4. EN 15804+A2
EN 15804+A2: 2019: Sustainability of construction works — Environmental Product Declarations — Core rules for the product category of construction products
5. Kiwa-Ecobility Experts (Kiwa-EE)
General Product Category Rules - Version 2.1, 2022-02-14
6. Institut Bauen und Umwelt e.V
Complementary Product Category Rule (c-PCR): Requirements on the EPD for Mineral factory-made mortar - 12/07/2023 v3
7. EPD Fjärrvärme för Linköpings fjärrvärmenät från Tekniska verken i Linköping AB, S-P-08296
8. University thesis: Cirkulär ekonomi för rivningsbetong Med fokus på återvinning , Chalmers Tekniska Högskola, Report number E2019:125
9. BBSR - The Federal Office for Building and Regional Planning: Nutzungsdauern von Bauteilen für Lebenszyklusanalysen nach Bewertungssystem Nachhaltiges Bauen (BNB) (Service
lives of building elements for Life Cycle Assessments conducted according to the BNB Sustainable Building assessment system), dated 24 February 2017
10. A Life Cycle Assessment of Silica Sand: Comparing the Beneficiation Processes. Anamarija Grbeš. Sustainability 2016, 8, 11.
11. EN 998-1:2016 General purpose plastering mortar (GP) CS III
12. NMD Determination Method V1.1 (March 2022)
StoLevell Evo | ReTHiNK-62142 18 / 19
Environmental Product Declaration
8 Contact information
Publisher Operator Owner of declaration
Kiwa-Ecobility Experts Kiwa-Ecobility Experts Sto SE & Co. KGaA
Voltastraße 5 Voltastraße 5 Ehrenbachstraße 1
13355 Berlin, DE 13355 Berlin, DE D-79780 Stühlingen, DE
E-mail: E-mail: E-mail:
DE.Ecobility.Experts@kiwa.com DE.Ecobility.Experts@kiwa.com infoservice@sto.com
Website: Website: Website:
https://www.kiwa.com/de/en/themes/ecobility-experts/ecobility-https://www.kiwa.com/de/en/themes/ecobility-experts/ecobility-https://www.sto.com
experts-epd-program/ experts-epd-program/
Kiwa-Ecobility Experts is
established member of the
StoLevell Evo | ReTHiNK-62142 19 / 19
