ENVIRONMENTAL-PRODUCT DECLARATION
as per ISO 14025 and EN 15804+A2
Owner of the Declaration Sika Services AG
Publisher Institut Bauen und Umwelt e.V. (IBU)
Programme holder Institut Bauen und Umwelt e.V. (IBU)
Declaration number EPD-SIK-20220221-IBA1-EN
Issue date 25/11/2022
Valid to 24/11/2027
Sikaplan VGWT
Sika Services AG
www.ibu-epd.com | https://epd-online.com
1. General Information
Sika Services AG Sikaplan VGWT
Programme holder Owner of the declaration
IBU – Institut Bauen und Umwelt e.V. Sika Services AG
Hegelplatz 1 Tüffenwies 16-22
10117 Berlin 8064 Zurich
Germany Switzerland
Declaration number Declared product / declared unit
EPD-SIK-20220221-IBA1-EN 1 m² Sikaplan VGWT polymeric waterproofing membrane
This declaration is based on the product category rules: Scope:
Plastic and elastomer roofing and sealing sheet systems, This document applies to Sikaplan VGWT polymeric waterproofing
01/08/2021 membrane manufactured by Sika Manufacturing AG in Duedingen,
(PCR checked and approved by the SVR) Switzerland. The life cycle assessment data are based on production data
from 2021 collected by Sika Services AG.
The owner of the declaration shall be liable for the underlying information
Issue date and evidence; the IBU shall not be liable with respect to manufacturer
information, life cycle assessment data and evidences.
25/11/2022
The EPD was created according to the specifications of EN 15804+A2. In
the following, the standard will be simplified as EN 15804 bezeichnet.
Valid to
24/11/2027 Verification
The standard EN 15804 serves as the core PCR
Independent verification of the declaration and data according to ISO
14025:2011
internally X externally
Dipl.-Ing Hans Peters
(chairman of Institut Bauen und Umwelt e.V.)
Florian Pronold Mrs Kim Allbury,
(Managing Director Institut Bauen und Umwelt e.V.) (Independent verifier)
1 Environmental-Product Declaration - Sika Services AG - Sikaplan VGWT
2. Product
• Directive no. xyz: date, title
2.1 Product description/Product definition
• Regulation no. xyz: date, title
Sikaplan VGWT is
• and the harmonised standards based on these
a multi-layer synthetic roof waterproofing sheet based on
provisions:
polyvinyl chloride
• EN xyz: date, title
(PVC) with embedded polyester scrim reinforcing (DE/E1 PVC-
The CE-marking takes into account the proof of conformity with
P-NB-V-PG).
the respective harmonized standards based on the legal
provisions above.
For the application and use the respective national provisions
Sikaplan VGWT waterproofing
apply.
sheets are available in these thicknesses: 1.2 mm, 1.5 mm and
1.8 mm.
[Alternative 2b: Product harmonized as well in accordance
with the CPR as with other provisions for harmonisation of
the EU]:
For the placing of the product on the market in the European
All values given in the LCIA results section apply to Sikaplan
Union/European Free Trade Association (EU/EFTA) (with the
VGWT-12; a formula
exception of Switzerland) the Regulation (EU) No. 305/2011/
for individually calculating values for other thicknesses is given
(CPR) and the following other provisions for harmonisation
in Chapter 5.
apply:
Placement of the product on the market in the European
• Directive (EU) xyz: date, title
Union/European Free Trade Association (EU/EFTA) (except for
• Regulation (EU) no. xyz: date, title
Switzerland) is subject to Regulation (EU) No. 305/2011 (CPR).
The product needs a declaration of performance in accordance
The product requires a Declaration of Performance in
with the CPR taking into consideration /EN xyz: date/, title or
accordance with the harmonised standard EN 13956:2012
/ETA no. xyz/:date, title respectively and the CE-marking.
“Flexible sheets for waterproofing” and the CE marking.
Application is subject to the regulations of each specific
The CE-marking for the product takes into account the
country; in Germany the application standard DIN SPEC
Declaration of Performance in accordance with the CPR and
20000-201.
the proof of conformity with the following harmonised standards
Please select one of the following options and delete the
or based on the other provisions for harmonisation:
header of the selected [alternative]:
• EN xyz: date, title
[Alternative 1a: Product according to the CPR based on a
• Source, date, title
hEN]:
For the application and use the respective national provisions
apply.
For the placing on the market of the product in the European
Union/European Free Trade Association (EU/EFTA) (with the
[Alternative 3: Product for which no legal provisions for
exception of Switzerland) Regulation (EU) No. 305/2011 (CPR)
harmonisation of the EU exist]:
applies. The product needs a declaration of performance taking
into consideration EN xyz:date, title and the CE-marking. For the use and application of the product the respective
national provisions at the place of use apply, in Germany for
For the application and use the respective national provisions
example the building codes of the federal states and the
apply.
corresponding national specifications.
[Alternative 1b: Products according to the CPR based on
an ETA]: 2.2 Application
Sikaplan VGWT
For the placing of the product on the market in the European waterproofing sheets are used mainly for waterproofing flat
Union/European Free Trade Association /EU/EFTA) (with the roofs. The sheets can
exception of Switzerland) the Regulation (EU) No. 305/2011 be loosely laid and mechanically fastened to roofs with any
(CPR) applies. The product needs a declaration of performance slope.
taking into consideration ETA no. xyz:date, title and the CE-
marking. 2.3 Technical Data
In the following table, only technical data
For the application and use the respective national provisions relevant to Sikaplan VGWT waterproofing sheets are given.
apply.
Technical data
[Alternative 2a: Product not harmonised in accordance
with the CPR but in accordance with other provisions for
harmonisation of the EU]:
For the placing on the market in the European Union/European
Free Trade Association (EU/EFTA) (with the exception of
Switzerland) the following legal provisions apply:
2 Environmental-Product Declaration - Sika Services AG - Sikaplan VGWT
Name Value Unit
Watertightness as per EN 1928 Passed
Sika maintains
Tensile strain as per EN 12311-2 ≥ 15 %
a quality management system certified in accordance with ISO
Peel resistance of the seam joint as
Passed - 9001.
per EN 12316-2
Shear resistance of the seam joint as 2.7 Environment and health during manufacturing
≥ 600 N/50mm
per EN 12317-2 In the production of Sikaplan VGWT polymeric waterproofing
Passed (> membrane, the regulatory standards for exhaust gasses, waste
Artificial ageing as per EN 1297 5000 h) - water and solid waste as well as for noise emissions are fully
met and the various limits are not exceeded. The health of
Dimensional stability as per EN 1107-2 ≤ |0.5| %
production personnel is not put at risk during production.
Folding in the cold as per EN 495-5 ≤ -30 °C
Waste gasses from the production process are collected and
Performance data of the product in accordance with the filtered in exhaust gas scrubbers.
declaration of performance with respect to its essential Water used is used exclusively for cooling and does not come
characteristics according to EN 13956:2012, Flexible sheets for into contact with the polymeric waterproofing membrane. There
waterproofing. are no hazardous goods according to the REACH listing.
2.4 Delivery status In addition to national requirements, there are Sika strategic
The products are delivered palletised: 20 m x 2 m or 20 m x goals for waste, energy and water reduction, as well as for zero
1.54 m, each 21 rolls per pallet. personal accidents at work. There are regular meetings with the
neighbourhood for feedback regarding, e.g. noise. Employees
2.5 Base materials/Ancillary materials
receive regular training for process standards, and for safety
The base materials and ancillary materials of Sikaplan VGWT and hazards.
polymeric waterproofing membrane are: Sika maintains an environmental management system
certified in accordance with ISO 14001.
• Polyvinyl chloride / PVC: 50 - 70% 2.8 Product processing/Installation
• Plasticiser (Phthalate): 34 - 40% Sikaplan VGWT polymeric
• Stabiliser (UV/Heat): 0 - 2% waterproofing sheets are loose laid with mechanical fastening
• Fire retardant (inorganic): 2 - 4% for unballasted
• Carrier (Polyester scrim): 1 - 3% roofs with any slope. Seams between sheets are hot-air
• Pigments: 0 - 8% welded; linear fastening
This product contains substances listed in the Candidate List of is recommended.
Substances of Very High Concern for Authorisation (SVHC)
(date: 04.07.2022) exceeding 0.1 percentage by mass: no
2.6 Manufacture
Sikaplan VGWT polymeric
waterproofing sheets are manufactured in the following steps:
In principle, the current product data sheet
should be consulted. Please request further information from
• Dosing of the various raw materials and plastification your local Sika organisation.
of the mixture in an extruder
2.9 Packaging
• Rolling the melt into sheets by calendar processing
• Cooling and reeling the sheets The rolls of polymeric waterproofing sheets are
• Heat fusing of two sheets (top and bottom layers), wrapped in PE stretch foil and shipped on pallets. The
embedding cardboard spools are
a polyester mesh, on a lamination machine made of recycled paper. The packaging materials can be sorted
• Trimming the sheets and winding them onto cardboard and collected for
spools made of recycled paper recycling.
• Wrapping the rolls in PE stretch film, palletising
2.10 Condition of use
Professionally installed and properly used, the
condition of Sikaplan VGWT polymeric waterproofing
membrane remains unchanged
throughout its service life. This was confirmed in 2005 by the
internal study Radar. Additionally, it was confirmed in the study
by the British Board of Agrément (BBA).
2.11 Environment and health during use
During their service life, Sikaplan VGWT synthetic
waterproofing sheets have no negative influence on the
environment and health
of users.
Production 2.12 Reference service life
waste such as scrap is recycled by feeding it directly back into
The reference
the
service life of Sikaplan VGWT synthetic waterproofing sheets is
manufacturing process.
at least 35 years.
The British Board of Agrément (BBA) certified Sikaplan
3 Environmental-Product Declaration - Sika Services AG - Sikaplan VGWT
VGWT to “under normal service conditions (…) provide a
durable roof 2.14 Re-use phase
waterproofing with a service life in excess of 35 years” At the end of the service life or when roofing
sheets must be replaced, Sikaplan VGWT waterproofing sheets
This can be selectively
conclusion reflects the high resistance to weathering and aging removed and recycled. This allows for a closed-loop material
of the product cycle.
when properly used. Sika
Description of the influences on the ageing of the product when Services AG is affiliated with Roofcollect, the recycling system
applied in accordance with the rules of technology. for polymeric
roofing and waterproofing membranes. This enables
increasingly more material
2.13 Extraordinary effects recovery from sorted polymeric waterproofing membranes.
Fire
Sikaplan VGWT polymeric 2.15 Disposal
waterproofing membrane is Sikaplan VGWT polymeric waterproofing sheets can be
classified in Construction Material Class E, as defined by EN recycled at the end of the use stage.
13501-1.
The sheets are completely recycled by Roofcollect
Fire protection
in numerous recycling systems and new products are
Name Value manufactured from the
Building material class E recovered material.
Burning droplets
Sikaplan VGWT polymeric waterproofing membrane
Smoke gas development
can be classified under Waste Code 170904 as defined by the
European Waste
Water Catalogue.
No environmental impact due to water exposure of the installed
Sikaplan VGWT polymeric waterproofing membrane is known. 2.16 Further information
More information about the company and its products is
Mechanical destruction available on the internet at www.sika.com.
Sikaplan VGWT polymeric waterproofing membrane Detailed information on the polymeric waterproofing
possesses good mechanical strength and is highly robust. No membranes is available at your local Sika organisation's
environmental impact website.
is known to result from unexpected mechanical damage.
3. LCA: Calculation rules
• A4: Transport to the building site
3.1 Declared Unit • A5: Installation into the building (welding energy,
This declaration applies to 1 m2 of Sikaplan VGWT polymeric disposal of packaging
waterproofing membrane, thickness 1.2 mm. A formula is given • C1: Deconstruction and demolition
for an independent calculation of the values for other • C2/1: Transport to the recycling facility
thicknesses. • C2/2: Transport to the incineration facility
• C3/1: Waste processing for recycling
Declared unit
• C3/2: Waste incineration
Name Value Unit
• C4: Disposal
Declared unit 1 m2 • D: Potential for reuse, recovery and/or recycling as net
Grammage 1.5 kg/m2 flows and benefits
Type of sealing Hot-air weld -
3.3 Estimates and assumptions
Layer thickness 0.0012 m
Various stabilisers were approximated with a
For IBU core EPDs (where clause 3.6 is part of the EPD): for general chemical dataset or proxies were built. The percentage
average EPDs, an estimate of the robustness of the LCA by mass is < 3 %.
values must be made, e.g. concerning variability of the
production process, geographical representativeness and the The membrane is assumed to be removed by hand at the end
influence of background data and preliminary products of life, so no
compared to the environmental impacts caused by actual inputs/outputs are considered.
production.
3.4 Cut-off criteria
All data were taken into account (recipe constituents, thermal
3.2 System boundary energy used, electricity used). Transport expenses were
Type of EPD: Cradle-to-gate with options considered for all inputs and outputs. The manufacturing of the
production machines and
The system boundaries of the EPD follow the modular systems and associated infrastructure was not taken into
construction system described by EN 15804+A2. The LCA account in the LCA. Additionally, inputs (solvents, lubricant oils)
takes into account the following modules: needed for maintenance of the production line, lighting, hygiene
related water
• A1-A3: Manufacturing of pre-products, packaging,
use, transportation of employees were considered negligible
ancillary materials, transport to the factory, production
and excluded
including energy supply and waste handling
4 Environmental-Product Declaration - Sika Services AG - Sikaplan VGWT
from the analysis. Land or region, in which the declared product system is
manufactured, used or handled at the end of the product´s
3.5 Background data lifespan: Switzerland
The primary data provided by Sika derive from the plant at
Duedingen, Switzerland. The underlying data were collected in
the databases of GaBi software (version CUP2022.1) and 3.9 Allocation
ecoinvent Version 3.8. The Swiss Electrical Energy Mix was Production waste that was reclaimed and reused
applied. internally has been modelled as closed-loop recycling
in Modules A1-A3.
3.6 Data quality Regarding the recycling of the polymeric waterproofingsheets,
To simulate the product stage, data recorded by Sika the amount of recyclable membrane was treated as a
from the production year 2021 were used. All other corresponding PVC benefit. Benefits for the disposal of
relevant background datasets were taken from generic packaging (incineration), scrap and roofing membrane are
data not older than 10 years, using as many as datasets credited in Module D; this also applies to the reuse of wooden
possible for raw pallets.
materials and processes with technological and geographical
representativeness. 3.10 Comparability
Basically, a comparison or an evaluation of EPD data is only
3.7 Period under review possible if all the data sets to be compared were created
The period under review is the year 2021. according to EN 15804 and the building context, respectively
the product-specific characteristics of performance, are taken
3.8 Geographic Representativeness
into account.
The used background database has to be mentioned.
4. LCA: Scenarios and additional technical information
Characteristic product properties
Information on biogenic carbon In case a reference service life according to applicable ISO
standards is declared then the assumptions and in-use
The biogenic carbon content quantifies the amount of biogenic conditions underlying the determined RSL shall be declared. In
carbon in a construction product leaving the factory gate, and it addition, it shall be stated that the RSL applies for the reference
shall be separately declared for the product and for any conditions only.
accompanying packaging.
If the total mass of biogenic carbon containing materials is less The same holds for a service life declared by the manufacturer.
than 5 % of the total mass of the product and accompanying Corresponding information related to in-use conditions needs
packaging, the declaration of biogenic carbon content may be not be provided if a service life taken from the list on service life
omitted. The mass of packaging containing biogenic carbon by BNB is declared.
shall always be declared.
Reference service life
Note: 1 kg of biogenic carbon is equivalent to 44/12 kg of CO2.
Name Value Unit
Reference service life 35 a
Information on describing the biogenic Carbon Content at
factory gate The British Board of Agrément (BBA) certified Sikaplan
VGWT to provide a durable roof
Name ValueUnit
waterproofing with a service life in excess of 35 years.
kg
Biogenic carbon content in product -
C
End of life (C1-C4)
Biogenic carbon content in accompanying kg
0.066
packaging C Name Value Unit
Recycling Scenario 1 100 %
The following technical information serves as a basis for the Transport to recycling (boat) 160 km
declared modules or can be used for the development of Transport to recycling (truck) 1240
specific scenarios in the context of a building assessment. Recycling Scenario 2 100 %
Transport to the building site (A4) Transport to incineration (truck) 500
Name Value Unit Reuse, recovery and/or recycling potentials (D), relevant
Litres of fuel (truck) 0.004 l/100km scenario information
Transport distance (truck) 1600 km The benefits from the incineration of waste produced during
installation are credited in Module D as avoided generation of
Gross density of products transported 1250 kg/m3
electricity and thermal energy, since in modern incineration
Transport distance (boat) 160 km
plants the energy of combustion is used to produce power and
Litres of fuel (boat) 0.0008 l/100km thermal energy. The membrane material recycled at the end-of-
life is credited as avoided production of PVC, while the partial
Installation into the building (A5)
reuse of pallets from packaging is also included in Module D as
Name Value Unit avoided production of new pallets.
Electricity consumption 0.016 kWh
Material loss (membrane) 2 %
Overlaps (membrane) 8 %
5 Environmental-Product Declaration - Sika Services AG - Sikaplan VGWT
5. LCA: Results
The results displayed below apply to Sikaplan VGWT-12. To calculate results for other thicknesses, please use
this formula:
I = ((x+0.58)/1.78) * I
x 1.2
[I = the unknown parameter value for Sikaplan VGWT products with a thickness of "x" mm (e.g. 1.5 mm)]
x
DESCRIPTION OF THE SYSTEM BOUNDARY (X = INCLUDED IN LCA; ND = MODULE OR INDICATOR NOT DECLARED; MNR =
MODULE NOT RELEVANT)
BENEFITS
AND LOADS
CONSTRUCTION
BEYOND
PRODUCT STAGE PROCESS USE STAGE END OF LIFE STAGE
THE SYSTEM
STAGE
BOUNDARIE
S
la ire ta m w a Ry lp p u s tro p s n a rT g n iru tc a fu n a M e h t m o rf tro p s n a rTe tis e h t o t e ta g y lb m e s s A e s U e c n a n e tn ia M ria p e R tn e m e c a lp e R tn e m h s ib ru fe R y g re n e la n o ita re p Oe s u re ta w la n o ita re p Oe s u n o itc u rts n o c -e Dn o itilo m e d tro p s n a rT g n is s e c o rp e ts a W la s o p s iD -e s u e R-y re v o c e R-g n ilc y c e Rla itn e to p
A1 A2 A3 A4 A5 B1 B2 B3 B4 B5 B6 B7 C1 C2 C3 C4 D
X X X X X MND MND MNR MNR MNR MND MND X X X X X
RESULTS OF THE LCA - ENVIRONMENTAL IMPACT according to EN 15804+A2: 1 m2 membrane
Parameter Unit A1-A3 A4 A5 C1 C2/1 C2/2 C3/1 C3/2 C4 D/1 D/2
GWP-total kg CO 2 eq 4.17E+00 5.49E-02 6.9E-01 0 1.95E-02 6.4E-03 2.34E-01 4.23E+00 0 -2.85E+00 -1.2E+00
GWP-fossil kg CO 2 eq 4.35E+00 5.48E-02 5.38E-01 0 2.56E-02 8.86E-03 2.3E-01 4.23E+00 0 -2.82E+00 -1.19E+00
GWP-
biogenic kg CO 2 eq -2.51E-01 5.04E-05 1.45E-01 0 -6.95E-03 -2.8E-03 3.69E-03 3.33E-03 0 -2.29E-02 -9.52E-03
GWP-luluc kg CO 2 eq 6.33E-02 7.24E-05 6.35E-03 0 8.46E-04 3.41E-04 2.65E-05 3.26E-04 0 -1.71E-03 -2.3E-04
kg CFC11
ODP 4.56E-09 4.79E-15 4.57E-10 0 9.3E-15 3.67E-15 1.65E-12 4.04E-12 0 -2E-10 -1.4E-11
eq
AP mol H+ eq 4.59E-02 1.37E-03 4.8E-03 0 2.27E-04 3.62E-05 1.83E-04 1.09E-03 0 -3.96E-03 -1.23E-03
EP-
kg P eq 3.14E-05 4.78E-08 3.19E-06 0 4.54E-07 1.83E-07 3.39E-07 1.03E-06 0 -6.36E-06 -2.86E-06
freshwater
EP-marine kg N eq 2.06E-03 3.5E-04 2.63E-04 0 5.24E-05 7.1E-06 6.68E-05 3.63E-04 0 -1.26E-03 -4.39E-04
EP-terrestrial mol N eq 2.13E-02 3.84E-03 2.78E-03 0 6.16E-04 9.46E-05 7.24E-04 4.51E-03 0 -1.39E-02 -4.66E-03
kg NMVOC
POCP 1.35E-02 9.82E-04 1.5E-03 0 1.68E-04 2.82E-05 1.62E-04 1.04E-03 0 -6.99E-03 -1.13E-03
eq
ADPE kg Sb eq 9.82E+01 6.85E-01 1.02E+01 0 2.07E+00 8.18E-01 9.99E-01 7.48E+00 0 -6.86E+01 -1.69E+01
ADPF MJ 6.25E-02 3.29E-09 6.25E-03 0 1.28E-08 5.12E-09 3.47E-08 9.89E-08 0 -5.55E-07 -3.24E-07
m3 world eq
WDP 3.59E-01 1.4E-04 6.32E-02 0 1.37E-03 5.49E-04 1.45E-02 3.25E-01 0 -1.09E-01 -1.62E-02
deprived
GWP = Global warming potential; ODP = Depletion potential of the stratospheric ozone layer; AP = Acidification potential of land and water; EP =
Eutrophication potential; POCP = Formation potential of tropospheric ozone photochemical oxidants; ADPE = Abiotic depletion potential for non-fossil
resources; ADPF = Abiotic depletion potential for fossil resources; WDP = Water (user) deprivation potential)
RESULTS OF THE LCA - INDICATORS TO DESCRIBE RESOURCE USE according to EN 15804+A2: 1 m2 membrane
Parameter Unit A1-A3 A4 A5 C1 C2/1 C2/2 C3/1 C3/2 C4 D/1 D/2
PERE MJ 1.22E+01 1.69E-02 1.78E-01 0 1.15E-01 4.65E-02 7.68E-01 1.99E+00 0 -8.94E+00 -6.53E+00
PERM MJ 1.75E+00 0 -3.34E-02 0 0 0 0 0 0 0 0
PERT MJ 1.39E+01 1.69E-02 1.45E-01 0 1.15E-01 4.65E-02 7.68E-01 1.99E+00 0 -8.94E+00 -6.53E+00
PENRE MJ 5.86E+01 6.86E-01 7.69E+00 0 2.08E+00 8.2E-01 4.26E+01 4.91E+01 0 -6.86E+01 -1.7E+01
PENRM MJ 4.05E+01 0 7.69E-01 0 0 0 -4.16E+01 -4.16E+01 0 0 0
PENRT MJ 9.91E+01 6.86E-01 8.46E+00 0 2.08E+00 8.2E-01 1E+00 7.49E+00 0 -6.86E+01 -1.7E+01
SM kg 5.45E-02 0 5.45E-03 0 0 0 0 0 0 -1.54E+00 0
RSF MJ 0 0 0 0 0 0 0 0 0 0 0
NRSF MJ 0 0 0 0 0 0 0 0 0 0 0
FW m3 2.55E-02 1.59E-05 3.24E-03 0 1.31E-04 5.26E-05 6.07E-04 8.47E-03 0 -1.18E-02 -2.67E-03
PERE = Use of renewable primary energy excluding renewable primary energy resources used as raw materials; PERM = Use of renewable primary
energy resources used as raw materials; PERT = Total use of renewable primary energy resources; PENRE = Use of non-renewable primary energy
excluding non-renewable primary energy resources used as raw materials; PENRM = Use of non-renewable primary energy resources used as raw
materials; PENRT = Total use of non-renewable primary energy resources; SM = Use of secondary material; RSF = Use of renewable secondary fuels;
NRSF = Use of non-renewable secondary fuels; FW = Use of net fresh water
RESULTS OF THE LCA – WASTE CATEGORIES AND OUTPUT FLOWS according to EN 15804+A2:
1 m2 membrane
Parameter Unit A1-A3 A4 A5 C1 C2/1 C2/2 C3/1 C3/2 C4 D/1 D/2
HWD kg 7.75E-07 2.94E-12 7.76E-08 0 9.91E-12 3.93E-12 1.04E-10 5.81E-10 0 -1.43E-06 -2.83E-09
6 Environmental-Product Declaration - Sika Services AG - Sikaplan VGWT
NHWD kg 2.15E-01 8.11E-05 7.19E-02 0 2.95E-04 1.17E-04 1.49E-02 2.58E+00 0 -3.3E-02 -1.06E-02
RWD kg 2.14E-03 7.47E-07 2.41E-04 0 2.55E-06 1.01E-06 8.6E-05 2.36E-04 0 -1.32E-03 -7.21E-04
CRU kg 0 0 0 0 0 0 0 0 0 0 0
MFR kg 0 0 0 0 0 0 1.54E+00 0 0 0 0
MER kg 0 0 0 0 0 0 0 0 0 0 0
EEE MJ 0 0 3.49E-01 0 0 0 1.14E-01 4.23E+00 0 0 0
EET MJ 0 0 6.29E-01 0 0 0 2.13E-01 7.72E+00 0 0 0
HWD = Hazardous waste disposed; NHWD = Non-hazardous waste disposed; RWD = Radioactive waste disposed; CRU = Components for re-use;
MFR = Materials for recycling; MER = Materials for energy recovery; EEE = Exported electrical energy; EET = Exported thermal energy
RESULTS OF THE LCA – additional impact categories according to EN 15804+A2-optional:
1 m2 membrane
Parameter Unit A1-A3 A4 A5 C1 C2/1 C2/2 C3/1 C3/2 C4 D/1 D/2
Disease
PM 4.72E+01 5.01E-01 4.97E+00 0 1.44E+00 5.68E-01 3.99E-01 6.29E+00 0 -3.47E+01 -3.25E+00
incidence
IR kBq U235 eq 1.95E-09 9.55E-12 2.03E-10 0 2.89E-11 1.14E-11 1.6E-11 2.5E-10 0 -9.64E-10 -1.87E-10
ETP-fw CTUe 3.52E-07 4.57E-10 3.58E-08 0 1.47E-09 5.83E-10 7.4E-10 2.67E-08 0 -3.68E-08 -8.29E-09
HTP-c CTUh 2.65E+01 8.18E-02 2.76E+00 0 6.98E-01 2.81E-01 5.26E-01 1.72E+00 0 -6.57E+00 -4.43E+00
HTP-nc CTUh 0 0 0 0 0 0 0 0 0 0 0
SQP SQP 0 0 0 0 0 0 0 0 0 0 0
PM = Potential incidence of disease due to PM emissions; IR = Potential Human exposure efficiency relative to U235; ETP-fw = Potential comparative
Toxic Unit for ecosystems; HTP-c = Potential comparative Toxic Unit for humans (cancerogenic); HTP-nc = Potential comparative Toxic Unit for humans
(not cancerogenic); SQP = Potential soil quality index
Disclaimer 1 – for the indicator “Potential Human exposure efficiency relative to U235”. This impact category deals mainly with the
eventual impact of low dose ionizing radiation on human health of the nuclear fuel cycle. It does not consider effects due to possible
nuclear accidents, occupational exposure nor due to radioactive waste disposal in underground facilities. Potential ionizing radiation
from the soil, from radon and from some construction materials is also not measured by this indicator.
Disclaimer 2 – for the indicators “abiotic depletion potential for non-fossil resources”, “abiotic depletion potential for fossil resources”,
“water (user) deprivation potential, deprivation-weighted water consumption”, “potential comparative toxic unit for ecosystems”,
“potential comparative toxic unit for humans – cancerogenic”, “Potential comparative toxic unit for humans - not cancerogenic”,
“potential soil quality index”. The results of this environmental impact indicator shall be used with care as the uncertainties on these
results are high or as there is limited experienced with the indicator.
6. LCA: Interpretation
The following chart shows the relative contributions of the energy use in a dominance analysis.
different modules to the various LCA categories and to primary
7 Environmental-Product Declaration - Sika Services AG - Sikaplan VGWT
biogenic, ODP, EP -
Examining freshwater and PERT. For GWP - biogenic, 12% of the impacts
the results for Sikaplan® VGWT, it can be concluded that the arise from the
most significant formulation and 87% of the impacts arise from the packaging.
contributor to the impact categories is the product stage For ODP, 26% of
(Module A1-A3). This the impacts arise from the formulation and 63% of the impacts
is true for all impact categories except GWP (total and fossil), arise from the
where packaging. For EP - freshwater, 66% of the impacts arise from
greenhouse gas emissions from the incineration of the the formulation
membrane in Module C3 of and 29% of the impacts arise from the packaging. For PERT,
Scenario 2 (100% Incineration) contribute to the results from 67% of the impacts
this impact arise from the formulation and 16% of the impacts arise from
category. The modules A1-A3 are further investigated in the the packaging.
following paragraphs. Within pre-product manufacturing, polymers play an important
role regarding GWP-total and GWP-fossil (38%), EP
Indicators of the inventory analysis: freshwater, marine and terrestrial (31 - 39%), WDP (21%) and
Due to electricity and natural gas use, the production process ADPF (41%). Plasticisers significantly influence GWP (33%),
(16%), pre-product manufacturing (67%) and packaging (16%) EP (21%), POCP (33%), WDP (32%) and ADPF (38%). Flame
account for most of the use of renewable primary energy retardants affect the AP (88%), ADPE (100%), POCP (22%)
resources (PERT). The manufacturing of polymers and and WDP (55%), and stabilisers affect the GWP-biogenic at
plasticisers in the production stage has the greatest impact highest contribution (100%), GWP-luluc (96%), ODP (89%) and
(96%) on the use of non-renewable primary energy resources EP-freshwater (55%). Pigments and fillers make a low
(PENRT), while the impact of the production process (energy) contribution to the impacts (below 7%). In addition, the carrier
is 3%. material contributes mostly to GWP-total and GWP-fossil
Indicators of the impact assessment: (15%), EP freshwater, marine and terrestrial (12 - 14 %) and
Examining ADPF (13%). The raw materials with the greatest overall effect
the results for module A1-3 in further detail, the raw materials on the impacts also show the greatest percentage by mass of
involved in the waterproofing membrane: polymers and plasticisers. The
the production of Sikaplan® VGWT represent greater than 86 manufacturing process (due to electricity use) contributes the
% across each of the most to ODP (11%), WDP (7%) and GWP-total (4%).
different impact categories. The exceptions are GWP -
7. Requisite evidence
8 Environmental-Product Declaration - Sika Services AG - Sikaplan VGWT
No requisite evidence is required for Sikaplan VGWT polymeric waterproofing membrane.
8. References
PCR, Part A sheets for roof waterproofing; German version EN 12310-
PCR, Part A: Institut Bauen und Umwelt e.V., Berlin (pub.): 2:2000.
Product Category Rules for Construction Products from the
range of Environmental Product Declarations of Institut Bauen
und Umwelt (IBU), Part A: Calculation Rules for the Life Cycle DIN EN 12311-2
Assessment and Requirements on the Background Report. DIN EN 12311-2: Flexible sheets for waterproofing -
2021. Determination of tensile properties - Part 2: Plastic and rubber
sheets for roof waterproofing; German version EN 12311-
2:2010.
PCR, Part B
DIN EN 12316-2
PCR, Part B: Requirements on the EPD for plastic and DIN EN 12316-2: Flexible sheets for waterproofing -
elastomer roofing and ceiling sheet systems, 2022. Determination of peel resistance of joints - Part 2: Plastic and
rubber sheets for roof waterproofing; German version EN
Regulation No. 305/2011 12316-2:2013.
Regulation No. 305/2011: of the European Parliament and of
the European Council laying down harmonised conditions for
the marketing of construction products and repealing Council DIN EN 12317-2
Directive 89/106/EEC. 9 March 2011. DIN EN 12317-2: Flexible sheets for waterproofing -
Determination of shear resistance of joints - Part 2: Plastic and
DIN EN 495-5 rubber sheets for roof waterproofing; German version EN
DIN EN 495-5: Flexible sheets for waterproofing - 12317-2:2010.
Determination of foldability at low temperature - Part 5: Plastic
and
rubber sheets for roof waterproofing; German version EN 495- DIN EN 13501-1+A1:2009
5:2013. DIN EN 13501-1+A1:2009: Fire classification of
construction products and building elements - Part 1:
DIN EN 1107-2 Classification
DIN EN 1107-2: Flexible sheets for waterproofing - using data from reaction to fire tests; German version EN
Determination of dimensional stability - Part 2: Plastic and 13501-1:2007+A1:2009.
rubber
sheets for roof waterproofing; German version EN 1107-2:2001.
DIN EN 13956
DIN EN 1297 DIN EN 13956: Flexible sheets for waterproofing -
DIN EN 1297: Flexible sheets for waterproofing - Plastic and rubber sheets for roof waterproofing - Definitions
Bitumen, plastic and rubber sheets for roof waterproofing - and
Method of characteristics; German version EN 13956:2012.
artificial ageing by long term exposure to the combination of
UV radiation, elevated temperature and water; German version EN 15804:2012+A2:2019:+AC:2021
EN 1297:2004. EN 15804:2012+A2:2019:+AC:2021:
Sustainability of construction works - Environmental product
DIN EN 1928 declarations - Core rules for the product category of
DIN EN 1928: Flexible sheets for waterproofing - construction
Bitumen, plastic and rubber sheets for roof waterproofing - products.
Determination of
watertightness; German version EN 1928:2000.
DIN SPEC 20000-201
DIN EN ISO 9001 DIN SPEC 20000-201: Use of building products
in construction works - Part 201: Adaption standard for flexible
sheets for waterproofing according to European standards for
DIN EN ISO 9001: Quality management systems - the use as
Requirements; trilingual version (German, English, French) EN waterproofing of roofs.
ISO 9001:2008-12.
DIN EN ISO 14001 British Board of Agrément (BBA)
British Board of Agrément (BBA), 2021 : Agrément
Certificate 09/4668
DIN EN ISO 14001: Environmental management systems - Product Sheet 4. Sika Waterproofing Membranes: Sikaplan G
Requirements with guidance for use; German and English and VG mechanically
version EN ISO fastened membranes - Sikaplan® VGWT.
14001:2004 + AC:2009.
DIN EN 12310-2 ecoinvent Version 3.8
DIN EN 12310-2: Flexible sheets for waterproofing - ecoinvent Version 3.8: Database for Life Cycle Assessment.
Determination of resistance to tearing - Part 2: Plastic and Swiss Centre for Life Cycle Inventories (ecoinvent Centre),
rubber 2021.
9 Environmental-Product Declaration - Sika Services AG - Sikaplan VGWT
REACH Candidate
European Waste Catalogue List: Candidate List of substances of very
European Waste Catalogue: European Waste Catalogue high concern for Authorisation: 04.07.2022.
Regulation, AVV, 2001.
Sphera: GaBi 10.6.1.35 and Database CUP 2022.1
Radar - Results from investigation into the condition of Sphera: GaBi 10.6.1.35 and Database CUP 2022.1: Software-
Sikaplan VGWT roofs after 15 and more years in use System and Databases for Life Cycle Engineering. Copyright,
Radar - Results from investigation into the condition of TM. Stuttgart, Echterdingen, 1992-2022.
Sikaplan VGWT roofs after 15 and more years in use: The literature referred to in the Environmental Product
Internal study by Sika Services AG, 2005. Declaration must be listed in full.Standards already fully quoted
in the EPD do not need to be listed here again.
The current version of PCR Part A and PCR Part B of the PCR
REACH Candidate document on which they are based must be referenced.
List
10 Environmental-Product Declaration - Sika Services AG - Sikaplan VGWT
Publisher
Institut Bauen und Umwelt e.V. +49 (0)30 3087748- 0
Hegelplatz 1 info@ibu-epd.com
10117 Berlin www.ibu-epd.com
Germany
Programme holder
Institut Bauen und Umwelt e.V. +49 (0)30 3087748- 0
Hegelplatz 1 info@ibu-epd.com
10117 Berlin www.ibu-epd.com
Germany
Author of the Life Cycle Assessment
Sika Technology AG +41 (0)58 436 40 40
Tüffenwies 16 product.sustainability@ch.sika.com
8048 Zürich www.sika.com/sustainability
Switzerland
Owner of the Declaration
Sika Services AG +41(0)58 436 40 40
Tüffenwies 16-22 product.sustainability@ch.sika.com
8064 Zurich https://www.sika.com/
Switzerland
11 Environmental-Product Declaration - Sika Services AG - Sikaplan VGWT
