ENVIRONMENTAL PRODUCT DECLARATION
as per ISO 14025 and EN 15804+A2
Owner of the Declaration Hilti Aktiengesellschaft
Publisher Institut Bauen und Umwelt e.V. (IBU)
Programme holder Institut Bauen und Umwelt e.V. (IBU)
Declaration number EPD-HIL-20230519-IBA1-EN
Issue date 22/11/2023
Valid to 21/11/2028
HIT-RE 500 V3
Hilti AG
www.ibu-epd.com | https://epd-online.com
1. General Information
Hilti AG HIT-RE 500 V3
Programme holder Owner of the declaration
IBU – Institut Bauen und Umwelt e.V. Hilti Aktiengesellschaft
Hegelplatz 1 Feldkircher Strasse 100
10117 Berlin 9494 Schaan
Germany Liechtenstein
Declaration number Declared product / declared unit
EPD­HIL­20230519­IBA1­EN The declared product is a HILTI injectable mortar HIT­RE 500 V3. The
declared unit is one kilogram of reaction resin product in the mixing ratio of
the two components necessary for processing. The packaging is also
included in the calculation. The declared unit is stated in [kg].
This declaration is based on the product category rules: Scope:
Reaction resin products, 01/08/2021 This document refers to the injectable mortar HIT­RE 500 V3 with its
(PCR checked and approved by the SVR) packaging. For the compilation of the life cycle assessment, specific data
were collected from the factory in Kaufering, Germany, of the HILTI AG.
Data from the year 2020 are used, which correspond to the annual
Issue date average.
The owner of the declaration shall be liable for the underlying information
22/11/2023
and evidence; the IBU shall not be liable with respect to manufacturer
information, life cycle assessment data and evidences.
Valid to
The EPD was created according to the specifications of EN 15804+A2. In
21/11/2028 the following, the standard will be simplified as EN 15804.
Verification
The standard EN 15804 serves as the core PCR
Independent verification of the declaration and data according to ISO
14025:2011
internally X externally
Dipl.­Ing. Hans Peters
(Chairman of Institut Bauen und Umwelt e.V.)
Florian Pronold Matthias Klingler,
(Managing Director Institut Bauen und Umwelt e.V.) (Independent verifier)
1 Environmental Product Declaration ­ Hilti AG ­ HIT­RE 500 V3
2. Product
The use of Hilti HDE­22 dispenser with Volume Calculator app
2.1 Product description/Product definition leads to no under or over fill, reducing underfilling related risks
The declared product of HIT­RE 500 V3 is a two­component and minimizing mortar wastage.
system. The resin component (component A) comprises a resin
based on epoxides as well as mineral fillers. The curing agent 2.3 Technical Data
component (component B) comprises of amine hardener,
Constructional data
mineral and cement­like fillers.
Name Value Unit
Mixing the two components A and B in the static mixer initiates Density EN ISO 1183­1 1420 kg/m3
the curing (hardening) reaction of both binder systems. During Compressive strength (Tcure=120h) EN
105 N/mm2
the curing phase, a very strong bond is formed between the ISO 604
organic and inorganic binder matrix. The system formed during Elastic modulus (pressure) EN ISO 604 4800 N/mm2
curing results in a cross­linked duromer with desired design
Tensile shear strength acc. to DIN EN not
properties (high bond strengths within defined curing time) and N/mm2
14293 relevant
particular long­term stability.
Tensile bond strength acc. to DIN EN not
N/mm2
Composite foils are used for the two­component foil pack of 14293 relevant
HIT­RE 500 V3. This kind of packaging serves the following Hilti HIT-RE 500 V3 displays the following characteristics:
purposes: waste volume reduction, easy storage and transport,
less packaging material. Performance data of the product in accordance with the
declaration of performance with respect to its essential
Through legislation and increased public awareness users have characteristics according to
increasingly become discerned towards the use of highly
volatile components with their resulting unpleasant odour and ETA 16/0142
low flash point (flammability). ETA 16/0143
ETA 16/0180
The reaction resins used in all Hilti adhesives are practically ETA 18/0745
odourless and have a considerably higher flash point, i.e. ETA-18/1022
higher than 100 °C in comparison to 34 °C for styrene­based ETA-19/0194
products. HIT­RE 500 V3 is the high­performance injectable ETA-20/0125
hybrid mortar with approvals for rebar connections and heavy­ ICC ESR-3814
duty anchoring.
Shelf life of 12 months:
For the placing of the product on the market in the European Substratetemperature during installation ­5 to +40 °C (internal
Union / European Free Trade Association (EU/EFTA) (with the method).
exception of Switzerland) the Regulation (EU) No. 305/2011
(CPR) applies. The product needs a declaration of performance Working time:
taking into consideration the following European Technical
Approvals ­5 to 0 °C 120 min
> 0 to +4 °C 120 min
ETA 16/0142 > 4 to +9 °C 120 min
ETA 16/0143 > 9 to +14 °C 90 min
ETA 16/0180 > 14 to +19 °C 60 min
ETA 18/0745 > 19 to +24 °C 30 min
ETA-18/1022 > 24 to +29 °C 20 min
ETA-19/0194 > 29 to +34 °C 15 min
ETA-20/0125 > 34 to +39 °C 12 min
40 °C 10 min
and the CE­marking. For the application and use the respective
national provisions apply. Curing time:
2.2 Application
­5 to 0 °C 168 h
Hilti HIT­RE 500 V3 serves for safely securing of threaded rods
> 0 to +4 °C 48 h
and post­installed rebar connections in cracked and uncracked
> 4 to +9 °C 24 h
concrete C20/25 to C50/60. HIT­RE 500 V3 is ETA (European
> 9 to +14 °C 16 h
Technical Assessment) and ICC (International Code Council)
> 14 to +19 °C 12 h
approved for seismic C1 and C2 category for anchoring and C1
> 19 to +24 °C 7 h
category for rebar.
> 24 to +29 °C 6 h
> 29 to +34 °C 5 h
Hilti HIT­RE­500 V3 is a component of the Hilti SAFEset
> 34 to +39 °C 4,5 h
concept. Hilti SAFEset is an approved system which makes
40 °C 4 h
anchor installation an easier, safer and faster process. It
significantly improves the robustness of fastening and 2.4 Delivery status
dramatically reduces the possibilities of error during installation. The product Hilti HIT­RE 500 V3 is available in foil­packages
As part of SAFEset HIT­RE 500 V3 can be installed with with a total of 330 ml, 500 ml and 1400 ml injectable mortar in
approved Hilti Hollow Drill bits and vacuum cleaners that drill the corresponding mixing ratio.
and clean the hole in one step for virtually dust­free installation.
2 Environmental Product Declaration ­ Hilti AG ­ HIT­RE 500 V3
2.5 Base materials/Ancillary materials
Hilti HIT­RE 500 V3 is supplied in the form of a dual component
film­wrapped pack comprising a resin component and a curing
agent component at a volume ratio of 3:1. The mixing ratio of
resin and curing agent components is automatically set during
the injection process. Product curing commences directly after
the components are mixed.
The product reviewed in this EPD contains the following
component volumes:
Resin component:
Illustration: Production process of the reaction resin
Epoxide resin mixture: 60 to 70 % by weight mixture
Mineral fillers: 30 to 40 % by weight
Other: < 5 % by weight
Curing agent component:
Amine hardener mixture: 60­70 % by weight
Mineral fillers: 15 to 25 % by weight
Cement: 10 to 20 % by weight
Other: <5 % by weight
This product article contains substances listed in the candidate
list (date: 29.08.2023) exceeding 0.1 percentage by mass: no.
This product contains other Carcinogenic, Mutagenic,
Reprotoxic (CMR) substances in categories 1A or 1B which are
not on the candidate list, exceeding 0.1 percentage by mass:
no. Illustration: Production process of the packaging
2.7 Environment and health during manufacturing
Biocide products were added to this construction product or it
has been treated with biocide products (this then concerns a The manufacturing plant of HIT­RE 500 V3, Hilti GmbH
treated product as defined by the (EU) Ordinance on Biocide Industriegesellschaft für Befestigungstechnik, Hiltistr. 6, 86916
Products No. 528/2012): no. Kaufering, Germany, is certified according to ISO 14001 which
defines international standards for sustainable environmental
2.6 Manufacture management. The production site is also certified in
All raw materials are sourced from Europe. The transport is accordance with DIN EN ISO 50001 Energy Management
exclusively by truck. Chemical mortars are usually two­ Systems.
component systems consisting of a binder and a hardener.
2.8 Product processing/Installation
The production of chemical mortars consists of a mixing
process and a filling process of the respective single The product is delivered with Instructions for Use explaining the
components (binder and hardener) and their subsequent union basic steps for installation:
to a two­component system (container). Here as well process
control technology is used to weigh and mix solid and liquid 1) For safe handling the precautionary measures described in
compounds according to specification. In the next step both the SDS (e.g. hand and eye protection) must be adhered to
well­mixed components run through an automized filling line in 2) Insert the cartridge into the black cassette
which each of the processed masses is 3) Screw on the mixing nozzle
filled into a tubular foil bag. Finally the single components are 4) Put the cassette into the dispenser system
united in one container. The two­pack foil bags are packed into 5) Discard the first trigger pulls
cardboard boxes and then finally shipped. The manufacturing 6) Fill 2/3 of the borehole with mortar
plant of HIT­RE 500 V3, Hilti GmbH Industriegesellschaft für 7) Set the fixing element
Befestigungstechnik, Hiltistr. 6, 86916 Kaufering, Germany, is
certified according to ISO 9001. The guideline defines After mixing the components and squeezing the mortar into the
international standards for quality and process management. borehole the fixing element has to be set within the working
time mentioned in Instructions for Use. After the curing time,
The following flowcharts illustrate the underlying production described as well in Instructions for Use, the mortar is ready to
process take up loads.
2.9 Packaging
Hilti HIT­RE 500 V3 is supplied in the form of a 2­foil­pack
system and thus leads to very little waste remaining after use
on the construction site. After curing, the product can be
disposed of with household waste. Full or only partially emptied
cartridges must be disposed of as special waste in accordance
with official regulations.
The outer packaging consisting of plastic foil and cardboard
boxes designed according to the product size can be recycled.
3 Environmental Product Declaration ­ Hilti AG ­ HIT­RE 500 V3
Packaging contaminated by the product must be disposed of in Systems comply with at least the requirements of the DIN EN
a safe manner in accordance with local/national regulations. 13501-1 standard for fire classes E and Efl. As cross­linked
For this EPD, the declared packaging is a weighted meanvalue epoxy­amine resins do not melt or drip, the resins do not
of all available packaging sizes. This results in a 151 g of contribute towards spreading fire. Apart from the common
packaging composed of 64 g of plastic, 84g of paper and combustion that produces carbon monoxide and carbon
cardboard, 3 g of aluminium. dioxide, fire gases can contain traces of various phenolic
compounds. Due to the quantities used, they only have a
2.10 Condition of use subordinate influence on the fire characteristics of a building
During the installation, the temperature of the base material structure in which they have been installed.
must be between ­5 °C and +40 °C . The temperature of the
Fire protection
product should be between +5 and +25 °C during storage and
+5 and 40 °C during usage. Hilti literature and official approvals Name Value
must always be considered. The two components of HIT­RE Building material class E/Efl
500 V3 are only for use in combination with the defined volume Burning droplets No performance assessed
ratio and under these conditions mentioned above to build up a
Smoke gas development No performance assessed
cross­linked filled duromer.
2.11 Environment and health during use Water
Refer to the Safety Data Sheet (SDS) for detailed information The cured product is chemically inert and insoluble in water.
on handling, storage as well as first aid, firefighting and HIT­RE 500 V3 is certified for use as an anchoring adhesive in
accidental release measures and disposal considerations. concrete for water treatment applications according to National
Following the given instructions helps to minimize the risk for Sanitation Foundation (US) NSF.
health and the environment.
Mechanical destruction
2.12 Reference service life It is recommended to use dust protection during the demolition
Hilti HIT­RE 500 V3 is exposed to a wide variety of of the cured chemical anchor.
environmental factors during the use phase. The anticipated
Reference Service Life depends on the specific installation 2.14 Re-use phase
situation and the product exposure scenario. The main factors The product cannot be re­used. After usage the product can be
influencing the period of use involve weathering as well as removed by demolition.
mechanical loads and chemical exposure. Hilti HIT­­RE 500 V3
2.15 Disposal
is exposed to a wide variety of environmental factors during the
use phase. The anticipated Reference Service Life depends on Uncured Hilti HIT­RE 500 V3 can be disposed of according to
thespecific installation situation and the product exposure the European waste code 08 04 09* or 20 01 27*. The built­in
scenario. The main factors influencing the period of use involve cured anchor can be disposed as construction waste for which
weathering as well as mechanical loads and chemical the European waste code 17 01 01 applies.
exposure.
2.16 Further information
2.13 Extraordinary effects Further information is available on request under
Fire anchor.hse@hilti.com and on the Hilti website: www.hilti.group
Even without any special fire safety features the Injection
3. LCA: Calculation rules
transport modes (sea, road).
3.1 Declared Unit
The declared product is a HILTI injection mortar HIT­RE 500 A3 – Manufacturing:
V3. The declared unit refers to one kilogram of reaction resin Production, supply and use of energy sources at the
product in the required mixing ratio of the two components. The manufacturing sites (electricity, biomass and natural gas).
packaging of 0,151 kg/kg of product is also included in the Green electricity from wind turbines is considered for the whole
calculation. The following table shows the data of the declared manufacturing process. Production and transport of production
unit. losses, final product packaging and other inputs.
Declared unit End­of­life of production waste (hazardous, non­hazardous and
recyclable), production losses and raw material packaging,
Name Value Unit
including waste and losses transportation, processing and
Declared unit 1 kg
disposal.
3.2 System boundary A4 – Transport (to construction site)
The type of the EPD is cradle to grave. The following Transportation of packaged products from the manufacturing
information modules are defined as system boundaries in this site to the construction site,
study: including potential in­betweens (retailer, workshop, etc.).
A1 – Raw material supply: A5 – Installation­Construction
Production and packaging of the raw materials to be supplied to Electricity consumption for drilling and injecting (in case of
the manufacturer. All processes are included from cradle to injection with electrical dispenser). Production of the
gate. construction losses. Provision and end­of­life of tools and
accessories for injectable mortars (manual or electrical
A2 – Transport (to manufacturing site): dispenser with or without battery and with cartridge holder).
Transportation of all the raw materials and their packaging End­of­life of hazardous construction losses and packaging
between their production site and the manufacturing site, for all (uncured mortar and soiled packaging) and non­hazardous
4 Environmental Product Declaration ­ Hilti AG ­ HIT­RE 500 V3
construction losses (cured mortar and unsoiled packaging):
including waste transportation, processing and disposal. 3.9 Allocation
The energy for manufacturing (A3) is supposed to be the same
C1 – Deconstruction/demolition as for another HITLI product, in which consumptions were
Diesel for building demolition. measured on the production line. No allocation was used for
this stage.
C2 – Transport (to waste processing) The used operating tools (stage A5), which are Hilti's manual or
Transportation to waste processing facility. electrical dispenser can be used to inject the HIT­RE 500 V3 as
well as other Hilti products. The part of the dispenser's impact
C4– Waste disposal allocated to the current product is based on the estimated total
Treatment and disposal of plastic to sanitary landfill. mass of injected product each dispenser can be used for. This
can be considered as a mass allocation.
For the environmental impact, the use of green electricity (stage
3.10 Comparability
A3) was calculated taking into account the residual electricity
mix for the remaining electricity. The proportion of the electricity Basically, a comparison or an evaluation of EPD data is only
demand covered by green electricity in the total electricity possible if all the data sets to be compared were created
demand is 100%. according to EN 15804 and the building context, respectively
the product­specific characteristics of performance, are taken
3.3 Estimates and assumptions into account.
In general, background data and elecricity mixes are chosen
and calculated country­specifically for the production
processes. In some cases, assumptions were made because of
a lack of primary or secondary data, in particular for the
following aspects:
• The synthesis way of raw materials which were not
available on the Ecoinvent database were used to
reconstruct these material's impact
• Some raw material's packaging composition and
transportation distances were estimated
• The energy consumption for production of the current
product (HIT­RE 500 V3) was assimilated to the energy
consumption measured on the production line of
another Hilti product, which has a very similar
manufacturing process
• Estimations were made to calculate the energy
consumption during installation
• The transportation scenario to the building site is based
on French transportation companies' statistics.
3.4 Cut-off criteria
All information modules considered were included in the
calculation in such detail that all requirements of EN 15804 are
met. The consumption of additional inputs such as lubricants,
oils or solvents used for manufacture is less than 5 % by weight
and therefore falls below the cut­off criterion of the total
calculation.
3.5 Background data
The source for background data for the LCA calculations is the
ecoinvent 3.8 database.
3.6 Data quality
For the compilation of the life cycle assessment, specific data
were collected from the factory Kaufering, in Germany, of the
HILTI AG from the year 2020. The background data from the
ecoinvent 3.8 database used was updated in the year 2021 and
is thus highly up­to­date. The mass of the different components
of the reactive resin mixture comes from the information in the
recipe. The data quality is classified as appropriate.
3.7 Period under review
Data from the year 2020 are used, which correspond to the
annual average.
3.8 Geographic Representativeness
Land or region, in which the declared product system is
manufactured, used or handled at the end of the product´s
lifespan: Germany
5 Environmental Product Declaration ­ Hilti AG ­ HIT­RE 500 V3
4. LCA: Scenarios and additional technical information
Installation into the building (A5)
Characteristic product properties of biogenic carbon
The declared product contains 84 g of paper and cardboard Name Value Unit
(outer packaging and user manual). Moreover, during the Electricity consumption 0.00036 kWh
production of one of the raw materials, biogenic carbon is Uncured mortar loss 0,04 kg
captured. Since only the packaging and one raw material
Cured mortar loss 0,03 kg
contain biogenic carbon, in addition to a neglectable part
Material loss 0.07 kg
contained in the raw materials' packaging, all the biogenic
carbon capture and release were cancelled to simplify the Hazardous waste (soiled packaging) 0,067 kg
model. The cancelled emission corresponds to 0,025 kg of Non­hazardous waste (unsoiled packaging) 0,084 kg
biogenic carbon (0,093 kg of CO ) for a cancelled capture of
2
End of life (C1-C4)
0,151 kg of biogenic carbon (0,553 kg of CO ).
2
Name Value Unit
The following scenarios were considered for the LCA
calculations: Fuel for building demolition 0,0437 MJ
Distance to sanitary landfill 50 km
Transport to the building site (A4)
Landfilling 1 kg
Name Value Unit
Transport distance 900 km
Vehicle type lorry 16­32 metric ton ­
Effective load 21 t
Maximum capacity 24 t
Consumption when unloaded 0,25 L/km
Consumption at fill capacity 0,38 L/km
Empty return rate 14 %
Effective consumption 0,019 L/tkm
6 Environmental Product Declaration ­ Hilti AG ­ HIT­RE 500 V3
5. LCA: Results
DESCRIPTION OF THE SYSTEM BOUNDARY (X = INCLUDED IN LCA; MND = MODULE OR INDICATOR NOT DECLARED; MNR
= MODULE NOT RELEVANT)
Benefits and
Construction loads beyond
Product stage Use stage End of life stage
process stage the system
boundaries
la ire ta m w a Ry lp p u s tro p s n a rT g n iru tc a fu n a M e h t m o rf tro p s n a rTe tis e h t o t e ta g y lb m e s s A e s U e c n a n e tn ia M ria p e R tn e m e c a lp e R tn e m h s ib ru fe R y g re n e la n o ita re p Oe s u re ta w la n o ita re p Oe s u n o itc u rts n o c ­e Dn o itilo m e d tro p s n a rT g n is s e c o rp e ts a W la s o p s iD ­e s u e R­y re v o c e R­g n ilc y c e Rla itn e to p
A1 A2 A3 A4 A5 B1 B2 B3 B4 B5 B6 B7 C1 C2 C3 C4 D
X X X X X MND MND MNR MNR MNR MND MND X X X X X
RESULTS OF THE LCA - ENVIRONMENTAL IMPACT according to EN 15804+A2: 1 kg HIT-RE 500 V3
Parameter Unit A1 A2 A3 A4 A5 C1 C2 C3 C4 D
GWP­total kg CO 2 eq 3.25E+00 4.95E­02 4.75E­01 7.17E­02 5.72E­01 4.02E­03 4.84E­03 0 1.14E­01 0
GWP­fossil kg CO 2 eq 3.1E+00 4.93E­02 4.43E­01 7.14E­02 5.58E­01 4.02E­03 4.82E­03 0 1.14E­01 0
GWP­
biogenic kg CO 2 eq 4.04E­02 1.71E­04 3.03E­02 2.48E­04 6.18E­03 3.65E­06 1.67E­05 0 2.85E­04 0
GWP­luluc kg CO 2 eq 1.06E­01 1.97E­05 9.51E­04 2.85E­05 7.62E­03 4E­07 1.93E­06 0 2.15E­06 0
ODP kg CFC11 eq 4.13E­07 1.14E­08 5.66E­08 1.65E­08 6.98E­08 8.59E­10 1.12E­09 0 3.1E­09 0
AP mol H+ eq 1.67E­02 1.4E­04 2.04E­03 2.03E­04 2.34E­03 4.17E­05 1.37E­05 0 7.63E­05 0
EP­
kg P eq 9.91E­04 3.37E­06 1.36E­04 4.88E­06 1.71E­04 1.27E­07 3.3E­07 0 8.58E­07 0
freshwater
EP­marine kg N eq 6.3E­03 2.86E­05 5.8E­04 4.14E­05 6.24E­04 1.85E­05 2.79E­06 0 2.14E­03 0
EP­terrestrial mol N eq 3.92E­02 3.1E­04 4.36E­03 4.49E­04 6.25E­03 2.03E­04 3.03E­05 0 3.07E­04 0
kg NMVOC
POCP 1.45E­02 1.19E­04 1.34E­03 1.73E­04 1.48E­03 5.57E­05 1.17E­05 0 1.12E­04 0
eq
ADPE kg Sb eq 4.46E­05 1.78E­07 1.75E­06 2.58E­07 7.85E­06 2.04E­09 1.74E­08 0 3.11E­08 0
ADPF MJ 5.8E+01 7.33E­01 8.32E+00 1.06E+00 6.46E+00 5.41E­02 7.17E­02 0 2.22E­01 0
m3 world eq
WDP 5.47E+00 3.43E­03 2.32E­01 4.97E­03 4.56E­01 1.45E­04 3.36E­04 0 2.3E­03 0
deprived
GWP = Global warming potential; ODP = Depletion potential of the stratospheric ozone layer; AP = Acidification potential of land and water; EP =
Eutrophication potential; POCP = Formation potential of tropospheric ozone photochemical oxidants; ADPE = Abiotic depletion potential for non­fossil
resources; ADPF = Abiotic depletion potential for fossil resources; WDP = Water (user) deprivation potential)
RESULTS OF THE LCA - INDICATORS TO DESCRIBE RESOURCE USE according to EN 15804+A2: 1 kg HIT-RE 500 V3
Parameter Unit A1 A2 A3 A4 A5 C1 C2 C3 C4 D
PERE MJ 1.36E+01 1.07E­02 4.56E­01 1.55E­02 1.07E+00 3.09E­04 1.04E­03 0 1.17E­02 0
PERM MJ 0 0 6.81E­01 0 4.77E­02 0 0 0 0 0
PERT MJ 1.36E+01 1.07E­02 1.14E+00 1.55E­02 1.11E+00 3.09E­04 1.04E­03 0 1.17E­02 0
PENRE MJ 3.77E+01 7.33E­01 5.64E+00 1.06E+00 4.82E+00 5.41E­02 7.17E­02 0 2.22E­01 0
PENRM MJ 2.07E+01 0 2.68E+00 0 1.68E+00 0 0 0 0 0
PENRT MJ 5.84E+01 7.33E­01 8.32E+00 1.06E+00 6.49E+00 5.41E­02 7.17E­02 0 2.22E­01 0
SM kg 1.74E­02 2.5E­04 8.31E­02 3.62E­04 8.7E­03 2.12E­05 2.44E­05 0 8.41E­05 0
RSF MJ 3.29E­04 2.75E­06 6.72E­03 3.98E­06 5.2E­04 6.91E­08 2.69E­07 0 3.83E­06 0
NRSF MJ 0 0 0 0 0 0 0 0 0 0
FW m3 1.3E­01 9.35E­05 5.66E­03 1.35E­04 1.09E­02 3.28E­06 9.14E­06 0 2.92E­04 0
PERE = Use of renewable primary energy excluding renewable primary energy resources used as raw materials; PERM = Use of renewable primary
energy resources used as raw materials; PERT = Total use of renewable primary energy resources; PENRE = Use of non­renewable primary energy
excluding non­renewable primary energy resources used as raw materials; PENRM = Use of non­renewable primary energy resources used as raw
materials; PENRT = Total use of non­renewable primary energy resources; SM = Use of secondary material; RSF = Use of renewable secondary fuels;
NRSF = Use of non­renewable secondary fuels; FW = Use of net fresh water
RESULTS OF THE LCA – WASTE CATEGORIES AND OUTPUT FLOWS according to EN 15804+A2:
1 kg HIT-RE 500 V3
Parameter Unit A1 A2 A3 A4 A5 C1 C2 C3 C4 D
HWD kg 2.93E­01 8.34E­04 4.17E­02 1.21E­03 1.85E­01 7.23E­05 8.16E­05 0 3.46E­04 0
NHWD kg 4.17E+00 1.48E­02 5.02E­01 2.15E­02 4.87E­01 5.08E­04 1.45E­03 0 1E+00 0
RWD kg 9.57E­05 5.05E­06 1.41E­05 7.31E­06 1.77E­05 3.81E­07 4.93E­07 0 1.47E­06 0
CRU kg 0 0 0 0 0 0 0 0 0 0
MFR kg 5.89E­03 2.3E­06 5.1E­02 3.33E­06 9.35E­02 7.2E­08 2.25E­07 0 1.21E­06 0
MER kg 1.52E­02 1.85E­08 1.11E­05 2.68E­08 1.07E­03 1.15E­09 1.81E­09 0 5.85E­09 0
EEE MJ 3.3E­02 1.6E­04 7.35E­03 2.31E­04 3.82E­03 2.12E­05 1.56E­05 0 4.53E­04 0
EET MJ 1.32E­01 6.64E­04 2.13E­02 9.62E­04 1.42E­02 2.15E­04 6.49E­05 0 1.22E­03 0
7 Environmental Product Declaration ­ Hilti AG ­ HIT­RE 500 V3
HWD = Hazardous waste disposed; NHWD = Non­hazardous waste disposed; RWD = Radioactive waste disposed; CRU = Components for re­use;
MFR = Materials for recycling; MER = Materials for energy recovery; EEE = Exported electrical energy; EET = Exported thermal energy
RESULTS OF THE LCA – additional impact categories according to EN 15804+A2-optional:
1 kg HIT-RE 500 V3
Parameter Unit A1 A2 A3 A4 A5 C1 C2 C3 C4 D
Disease
PM 1.59E­07 3.97E­09 2.34E­08 5.75E­09 2.35E­08 1.12E­09 3.88E­10 0 1.62E­09 0
incidence
IR kBq U235 eq 2.5E­01 3.85E­03 3.51E­02 5.58E­03 3.22E­02 2.48E­04 3.76E­04 0 1.48E­03 0
ETP­fw CTUe 1.6E+02 6.12E­01 6.49E+00 8.87E­01 2.02E+01 3.25E­02 5.98E­02 0 4.83E­01 0
HTP­c CTUh 6.09E­09 1.88E­11 2.3E­10 2.73E­11 6.71E­10 1.25E­12 1.84E­12 0 7.12E­12 0
HTP­nc CTUh 8.99E­06 5.99E­10 1.09E­08 8.68E­10 6.33E­07 2.35E­11 5.86E­11 0 1.81E­10 0
SQP SQP 4.48E+01 5.21E­01 4.43E+00 7.55E­01 3.98E+00 7.03E­03 5.09E­02 0 5.83E­01 0
PM = Potential incidence of disease due to PM emissions; IR = Potential Human exposure efficiency relative to U235; ETP­fw = Potential comparative
Toxic Unit for ecosystems; HTP­c = Potential comparative Toxic Unit for humans (cancerogenic); HTP­nc = Potential comparative Toxic Unit for humans
(not cancerogenic); SQP = Potential soil quality index
Disclaimer 1 – for the indicator “Potential Human exposure efficiency relative to U235”. This impact category deals mainly with the
eventual impact of low­dose ionizing radiation on human health of the nuclear fuel cycle. It does not consider effects due to possible
nuclear accidents, occupational exposure or radioactive waste disposal in underground facilities. Potential ionizing radiation from the
soil, radon and from some construction materials is also not measured by this indicator.
Disclaimer 2 – for the indicators “abiotic depletion potential for non­fossil resources”, “abiotic depletion potential for fossil resources”,
“water (user) deprivation potential, deprivation­weighted water consumption”, “potential comparative toxic unit for ecosystems”,
“potential comparative toxic unit for humans – cancerogenic”, “Potential comparative toxic unit for humans ­ not cancerogenic”,
“potential soil quality index”. The results of this environmental impact indicator shall be used with care as the uncertainties on these
results are high as there is limited experience with the indicator.
6. LCA: Interpretation
The dominance analysis shows that the main causes of In the information module A1, the material supply of the resin
environmental impacts and indicators can be found in the mixture causes more than 70% of the global warming potential.
information module A1. This shows the global warming potential
for the provision of material with about 70 %, based on all
information modules. Modules A3 and A5 also represent an
important part of the final impact.
Illustration: Dominance analysis A1
The mass of the resin mixture come from the recipe information
provided by the manufacturer. According to the manufacturer,
this information can be assumed to be highly accurate.
Illustration: Dominance analysis A1- C4
The relevant datasets used to calculate the material availability
Module A1 is detailed below. Module A3's global warming of the product are topical with corresponding data in the latest
impact is mostly constituted by the final product packaging (9% Ecoinvent database (2021). The locations were also respected.
of the total impact). Most of the global warming impact from
module A5 is caused by the product losses (6% of the final Since these datasets strongly influence the results, as shown
impact) the end­of­life of the soiled product packaging, treated by the dominance analysis, so does the overall computation.
as hazardous waste (4% of the final impact).
7. Requisite evidence
Hilti HIT­RE 500 V3 complies with the requirements of in accordance with Eurofins test report, No. 392-2023-
00192602_A_EN and Eurofins test report, No. 392-2023-
• DIBt (2010) in combination with the NIK values from
0019602_H_EN respectively.
AgBB (2021) for applications in interior areas,
• emission class A+ outlined in the French VOC Directives AgBB overview of results (28 days [µg/m³])
(2020) in accordance with the Eurofins attestation,
• CDPH/EHLB Standard Method V 1.2 (2017)
8 Environmental Product Declaration ­ Hilti AG ­ HIT­RE 500 V3
Name Value Unit
TVOC (C6 ­ C16) <1000 μg/m3
Sum SVOC (C16 ­ C22) <100 μg/m3
R (dimensionless) <1 ­
VOC without NIK <100 μg/m3
Carcinogenic Substances <1 μg/m3
8. References
Standards
PCR Part B
DIN EN 13501-1 Institut Bauen und Umwelt e.V, Berlin (pub.): Product Category
Klassifizierung von Bauprodukten und Bauarten zu ihrem Rules for Construction Products from the range of
Brandverhalten Environmental Product Declarations for Institut Bauen und
Umwelt (IBU), Part B: Requirements on the EPD for Reaction
DIN EN 14293 resin products, 01.2019
Klebstoffe ­ Klebstoffe für das Kleben von Parkett auf einen
Untergrund ­ Prüfverfahren Regulation (EU) No. 305/2011 (CPR)
und Mindestanforderungen Regulation (EU) No 305/2011 of the European Parliament and
of the Council of 9 March 2011 laying down harmonised
DIN EN ISO 50001 conditions for the marketing of construction products and
DIN EN ISO 50001: 2018 Energy management systems ­ repealing Council Directive 89/106/EEC Text with EEA
Requirements with guidance for use relevance
EN 15804 Further References
EN 15804:2012+A1:2013, Sustainability of construction works
— Environmental Product Declarations — Core rules for the AFNOR, «FD P01-015» 2006
product category of construction products. Qualité environnementale des produits de construction ­
Fascicule de données énergie et transport
EN 15804
EN 15804:2012+A2:2019, Sustainability of construction works AgBB (2021)
— Environmental Vorgehensweise bei der gesundheitlichen Bewertung der
Product Declarations — Core rules for the product category of Emissionen von flüchtigen organischen Verbindungen (VVOC,
construction products. VOC und SVOC) aus Bauprodukten (2021)
EN ISO 604 Candidate List of substances of very high concern for
DIN EN ISO 604:2003­12: Determination of compressive Authorisation
properties European Cheminals Agency (ECHA), in accordance with
Article 50(10) of the REACH regulation
EN ISO 1183-1
DIN 51757:2011­01 Plastics ­ Methods for determining the CDPH/EHLB/Standard Method V1.2
density of non­cellular plastics ­ Part 1: Immersion method, California CDPH Standard Method is a US standard for
liquid pyknometer method and titration method evaluating and restricting VOC emissions to indoor air.
Developed in California as "Section 01350" Specification,
ISO 9001 several systems in the US refer to CDPH Standard Method
ISO 9001:2015 Quality management systems ­ Requirements
Comité National Routier (CNR)
ISO 14001 Enquête longue distance, PARIS, 2019
ISO 14001:2015 Environmental management systems ­
Requirements with guidance for use DIBt (2010)
Grundsätze zur gesundheitlichen Bewertung von Bauprodukten
ISO 14025 in Innenräumen (Oktober 2010)
EN ISO 14025:2011, Environmental labels and declarations —
Type III environmental declarations — Principles and Eurofins test report, No. 392-2023-0019602_A_EN
procedures. VOC test report for verification of compliance with
DIBt(2010)/AgBB(2018)
Ordinance on Biocide Products No. 528/2012 and with the French VOC directive from 2020
Regulation (EU) No 528/2012 of the European Parliament and
the Council of 22 May 2012 concerning the making available on Eurofins test report, No. 392-2023-0019602_H_EN
the market and use of biocidal products VOC test report for verification of compliance with
CDPH/EHLB/Standard Method V1.2 from 2017
PCR Part A
Institut Bauen und Umwelt e.V, Berlin (pub.): Product Category European Waste code
Rules for Construction Products from the range of in accordance with the European Waste Catalogue (EWC)
Environmental Product Declarations for Institut Bauen und (EWC 2014/955/EU) Commission
Umwelt (IBU), Part A: Calculation Rules for the Life Cycle Decision amending Decision 2000/532/EC on the list of waste
Assessment and Requirements on the Project pursuant to Directive 2008/98/EC of the European Parliament
Report according to EN 15804+A2:2019, 2021­04 and of the Council
9 Environmental Product Declaration ­ Hilti AG ­ HIT­RE 500 V3
peintures et vernis sur leurs émissions de polluants volatils
ETA 16/0142
European Technical Approval Hilti HIT­RE 500 V3 ICC ESR-3814
International code council (ICC), Evaluation report ESR4868
ETA 16/0143 HILTI HIT­RE 500 V3 (January 2023)
European Technical Approval Hilti HIT­RE 500 V3
NSF
ETA 16/0180 NSF/ANSI/CAN 61 Drinking Water System Components ­
European Technical Approval Hilti HIT­RE 500 V3 Health Effects
ETA 18/0745 Umwelt Bundesamt 2021
European Technical Approval Hilti HIT­RE 500 V3 Umwelt Bundesamt: Herkunftsnachweisregister (HKNR) —
Entwertungsnachweis durch
ETA-18/1022 GETECH ENERGIE GMBH für HILTI
European Technical Approval Hilti HIT­RE 500 V3
Database Ecoinvent 3.8
ETA-19/0194 ecoinvent Version 3
European Technical Approval Hilti HIT­RE 500 V3 Wernet, G., Bauer, C., Steubing, B., Reinhard, J., Moreno­Ruiz,
E., and Weidema, B., 2016. The ecoinvent database version 3
ETA-20/0125 (part I): overview and methodology. The International Journal of
European Technical Approval Hilti HIT­RE 500 V3 Life Cycle Assessment, [online] 21(9), pp.1218–1230. Available
at: [Accessed in 2021/2022].
French VOC Directives
Décret no 2011­321 du 23 mars 2011 relatif à l'étiquetage des Publication IBU 2021
produits de construction ou de Institut Bauen und Umwelt e.V.: General Instructions for the
revêtement de mur ou de sol et des peintures et vernis sur EPD programme of Institut Bauen und Umwelt e.V., Version
leurs émissions de polluants volatils 2.0, Berlin: Institut Bauen und Umwelt e.V., 2021
Arrêté du 19 avril 2011 relatif à l'étiquetage des produits de www.ibu­epd.com
construction ou de revêtement de mur ou de sol et des
10 Environmental Product Declaration ­ Hilti AG ­ HIT­RE 500 V3
Publisher
Institut Bauen und Umwelt e.V. +49 (0)30 3087748­ 0
Hegelplatz 1 info@ibu­epd.com
10117 Berlin www.ibu­epd.com
Germany
Programme holder
Institut Bauen und Umwelt e.V. +49 (0)30 3087748­ 0
Hegelplatz 1 info@ibu­epd.com
10117 Berlin www.ibu­epd.com
Germany
Author of the Life Cycle Assessment
ESTEANA +33 (0)9 53 23 98 30
Rue Mège 26 contact@esteana.fr
83220 Le Pradet www.esteana.fr
France
Owner of the Declaration
Hilti Aktiengesellschaft +423 234 2111
Feldkircher Strasse 100 HAGHSE@hilti.com
9494 Schaan www.hilti.com
Liechtenstein
11 Environmental Product Declaration ­ Hilti AG ­ HIT­RE 500 V3
