ENVIRONMENTAL PRODUCT DECLARATION
as per ISO 14025 and EN 15804+A2
Owner of the Declaration dormakaba International Holding GmbH
Publisher Institut Bauen und Umwelt e.V. (IBU)
Programme holder Institut Bauen und Umwelt e.V. (IBU)
Declaration number EPD-DOR-20220160-CBA1-EN
Issue date 11.10.2022
Valid to 10.10.2027
ITS 915/ITS 900
dormakaba
www.ibu-epd.com | https://epd-online.com
General Information
dormakaba ITS 915/ITS 900
Programme holder Owner of the declaration
IBU – Institut Bauen und Umwelt e.V. dormakaba International Holding GmbH
Hegelplatz 1 DORMA Platz 1
10117 Berlin 58256 Ennepetal
Germany Germany
Declaration number Declared product / declared unit
EPD-DOR-20220160-CBA1-EN 1 door closer (1 piece) of the ITS 915/ITS 900 including slide channel and
accessories
This declaration is based on the product category rules: Scope:
Building Hardware products, 01.08.2021 This Environment Product Declaration refers to a specific door closer
(PCR checked and approved by the SVR) manufactured by dormakaba Production GmbH & Co. KG. The production
site is located in Singapore.
Issue date The data represents the year 2020.
The owner of the declaration shall be liable for the underlying information
11.10.2022
and evidence; the IBU shall not be liable with respect to manufacturer
information, life cycle assessment data and evidences.
Valid to
The EPD was created according to the specifications of EN 15804+A2. In
10.10.2027 the following, the standard will be simplified as EN 15804.
Verification
The standard EN 15804 serves as the core PCR
Independent verification of the declaration and data according to ISO
14025:2011
internally X externally
Dipl.-Ing. Hans Peters
(Chairman of Institut Bauen und Umwelt e.V.)
Florian Pronold Dr.-Ing. Wolfram Trinius,
(Managing Director Institut Bauen und Umwelt e.V.) (Independent verifier)
1 Environmental Product Declaration - dormakaba - ITS 915/ITS 900
Product
Product description/Product definition Base materials/Ancillary materials
ITS 915/ITS 900 cam-action door closer is designed and The major material compositions including the packaging of the
manufactured to high quality standards to meet the growing product are listed below:
demand for an economical solution of high performance Name Value Unit
concealed overhead door closer with standard features. As a
Steel 53 %
concealed door closer ITS 915/900 can be installed directly in
Aluminum 29 %
the door or frame, making it virtually invisible. The compact
design of the closer body and slide-channel allow the door to Paper 10 %
maintain a high level of integrity. For the use and application of Lubricant 4 %
the product the respective national provisions at the place of Plastics 1 %
use apply. The standards which can be applied are the
Zinc 1 %
following:
Paint 1 %
• EN 1154 (only ITS 915)
Others 1 %
• UL/cUL listed
The product/s include/s partial articles which contain
Application substances listed in the Candidate List of REACH Regulation
The door closers can be easily installed in virtually all doors 1907/2006/EC (date: 17.01.2022) exceeding 0.1 percentage by
with a leaf thickness of 45 mm or more, while they can operate mass: yes
doors up to 1100 mm with the same mounting position. They
• Lead (Pb): 7439-92-1 (CAS-No.) is included in some of
offer easy adjustment with two independent valves.
the alloys used. The concentration of lead in each
individual alloy does not exceed 4.0% (by mass).
Technical Data
The Candidate List can be found on the ECHA website
The door closers have the following technical properties:
address: https://echa.europa.eu/de/home.
Reference service life
The reference service life of the ITS 915/ITS 900 door closers
depend on the traffic pattern and degree of usage of the door.
These closers are rated to EN 1154, meaning they are
designed to withstand a minimum of 500,000 cycles. The
reference service life amounts to 20 years. This corresponds
with approx. 25,000 cycles per year.
*EN 1154 only applicable for ITS 915. Performance data of the
product with respect to its characteristics in accordance with the
relevant technical provision which can be applied are
mentioned above.
2 Environmental Product Declaration - dormakaba - ITS 915/ITS 900
LCA: Calculation rules
final residues during the construction process stage.
Declared Unit
The declared unit is 1 piece of the product: ITS 915/ITS 900. End-of-life stage– Modules C1-C4 and D
Declared unit The end-of-life stage includes:
— C1, de-construction, demolition:
Name Value Unit
— C2, transport to waste processing;
Declared unit 1 piece/product
— C3, waste processing for reuse, recovery and/or recycling;
Mass of declared Product 1.98 kg — C4, disposal;
including provision and all transport, provision of all materials,
System boundary products and related energy and water use.
The type of EPD is: cradle to gate with options, modules C1–
C4, and module D (A1–A3 + C + D and additional modules: A4 Module D (Benefits and loads beyond the system boundary)
+ A5) includes:
— D, recycling potentials, expressed as net impacts and
Production - Module A1-A3 benefits.
The product stage includes:
Geographic Representativeness
— A1, raw material extraction, processing and mechanical
Land or region, in which the declared product system is
treatments, processing of secondary material input (e.g.
manufactured, used or handled at the end of the product´s
recycling processes), — A2, transport to the manufacturer,
lifespan: Singapore
— A3, manufacturing and assembly including provision of all
materials, products and energy, as well as waste processing up
to the end-of waste state.
Comparability
Basically, a comparison or an evaluation of EPD data is only
Construction stage - Modules A4-A5
possible if all the data sets to be compared were created
The construction process stage includes:
according to EN 15804 and the building context, respectively
— A4, transport to the building site;
the product-specific characteristics of performance, are taken
— A5, installation into the building;
into account.
including provision of all materials, products and energy, as well
as waste processing up to the end-of waste state or disposal of
LCA: Scenarios and additional technical information
Installation into the building (A5)
Characteristic product properties of biogenic carbon
Name ValueUnit
Information on describing the biogenic Carbon Content at
Output substances following waste treatment on
factory gate 0.25 kg
site (packaging)
Name ValueUnit
kg End of life (C1-C4)
Biogenic carbon content in product 0.01
C C1: The product dismantling from the building is done manually
Biogenic carbon content in accompanying kg without environmental burden.
0.09
packaging C C2: Transport to waste treatment at end of life is 50km.
Note: 1 kg of biogenic carbon is equivalent to 44/12 kg of CO . Name Value Unit
2
Recycling 4.12 kg
Reuse, recovery and/or recycling potentials (D), relevant
Additional technical information for the declared modules.
scenario information
Transport to the building site (A4)
Name Value Unit
Name Value Unit
Recycling 100 %
Litres of fuel truck (per piece) 0.00276l/100km
Collection rate is 100%.
Transport distance via truck 3500 km
Capacity utilisation (including empty runs)
55 %
average
Transport distance via ship 18000 km
3 Environmental Product Declaration - dormakaba - ITS 915/ITS 900
LCA: Results
DESCRIPTION OF THE SYSTEM BOUNDARY (X = INCLUDED IN LCA; MND = MODULE OR INDICATOR NOT DECLARED; MNR
= MODULE NOT RELEVANT)
Benefits and
Construction loads beyond
Product stage Use stage End of life stage
process stage the system
boundaries
la ire ta m w a Ry lp p u s tro p s n a rT g n iru tc a fu n a M e h t m o rf tro p s n a rTe tis e h t o t e ta g y lb m e s s A e s U e c n a n e tn ia M ria p e R tn e m e c a lp e R tn e m h s ib ru fe R y g re n e la n o ita re p Oe s u re ta w la n o ita re p Oe s u n o itc u rts n o c -e Dn o itilo m e d tro p s n a rT g n is s e c o rp e ts a W la s o p s iD -e s u e R-y re v o c e R-g n ilc y c e Rla itn e to p
A1 A2 A3 A4 A5 B1 B2 B3 B4 B5 B6 B7 C1 C2 C3 C4 D
X X X X X MND MND MNR MNR MNR MND MND X X X X X
RESULTS OF THE LCA - ENVIRONMENTAL IMPACT according to EN 15804+A2: 1 door closer
Parameter Unit A1-A3 A4 A5 C1 C2 C3 C4 D
GWP-total kg CO 2 eq 1.03E+01 7.23E-01 2.68E-01 0 8E-03 4.4E-02 2E-03 -4.23E+00
GWP-fossil kg CO 2 eq 1.06E+01 6.96E-01 7E-03 0 8E-03 4.4E-02 2E-03 -4.22E+00
GWP-biogenic kg CO 2 eq -3.04E-01 2.7E-02 2.61E-01 0 3.48E-04 1.02E-06 6.82E-06 -1.3E-02
GWP-luluc kg CO 2 eq 5E-03 1.62E-05 4.41E-06 0 1.79E-07 2.47E-06 5.75E-06 -6.28E-04
ODP kg CFC11 eq 1.25E-11 7.22E-17 4.83E-17 0 7.94E-19 2.2E-17 7.4E-18 -2.93E-11
AP mol H+ eq 4.79E-02 5E-03 7.5E-05 0 7.53E-06 7.77E-06 1.43E-05 -1.5E-02
EP-freshwater kg P eq 1.29E-05 1.5E-07 9.44E-09 0 1.61E-09 3.51E-09 3.43E-09 -2.32E-06
EP-marine kg N eq 7.23E-03 1E-03 2.71E-05 0 2.4E-06 1.75E-06 3.69E-06 -2E-03
EP-terrestrial mol N eq 8.4E-02 1.4E-02 3.38E-04 0 2.66E-05 3.54E-05 4.05E-05 -2.2E-02
kg NMVOC
POCP 2.36E-02 4E-03 7.18E-05 0 6.77E-06 4.85E-06 1.12E-05 -7E-03
eq
ADPE kg Sb eq 1.77E-04 2.04E-08 7.63E-10 0 2.26E-10 3.02E-10 1.79E-10 -3.81E-05
ADPF MJ 1.29E+02 9.63E+00 8.5E-02 0 1.07E-01 2E-02 2.6E-02 -5.77E+01
m3 world eq
WDP 1.37E+00 1E-03 3.3E-02 0 1.47E-05 4E-03 2.09E-04 -2.19E-01
deprived
GWP = Global warming potential; ODP = Depletion potential of the stratospheric ozone layer; AP = Acidification potential of land and water; EP =
Eutrophication potential; POCP = Formation potential of tropospheric ozone photochemical oxidants; ADPE = Abiotic depletion potential for non-fossil
resources; ADPF = Abiotic depletion potential for fossil resources; WDP = Water (user) deprivation potential)
RESULTS OF THE LCA - INDICATORS TO DESCRIBE RESOURCE USE according to EN 15804+A2: 1 door closer
Parameter Unit A1-A3 A4 A5 C1 C2 C3 C4 D
PERE MJ 3.36E+01 3.1E-02 2.28E+00 0 3.36E-04 1.15E-01 3E-03 -2.5E+01
PERM MJ 2.38E+00 0 -2.27E+00 0 0 -1.1E-01 0 0
PERT MJ 3.6E+01 3.1E-02 1.5E-02 0 3.36E-04 5E-03 3E-03 -2.5E+01
PENRE MJ 1.29E+02 9.63E+00 8.5E-02 0 1.07E-01 7.78E-01 2.6E-02 -5.78E+01
PENRM MJ 7.57E-01 0 0 0 0 -7.57E-01 0 0
PENRT MJ 1.29E+02 9.63E+00 8.5E-02 0 1.07E-01 2E-02 2.6E-02 -5.78E+01
SM kg 8E-01 0 0 0 0 0 0 0
RSF MJ 0 0 0 0 0 0 0 0
NRSF MJ 0 0 0 0 0 0 0 0
FW m3 8E-02 5.49E-05 7.82E-04 0 6.03E-07 1.07E-04 6.61E-06 -4.5E-02
PERE = Use of renewable primary energy excluding renewable primary energy resources used as raw materials; PERM = Use of renewable primary
energy resources used as raw materials; PERT = Total use of renewable primary energy resources; PENRE = Use of non-renewable primary energy
excluding non-renewable primary energy resources used as raw materials; PENRM = Use of non-renewable primary energy resources used as raw
materials; PENRT = Total use of non-renewable primary energy resources; SM = Use of secondary material; RSF = Use of renewable secondary fuels;
NRSF = Use of non-renewable secondary fuels; FW = Use of net fresh water
RESULTS OF THE LCA – WASTE CATEGORIES AND OUTPUT FLOWS according to EN 15804+A2:
1 door closer
Parameter Unit A1-A3 A4 A5 C1 C2 C3 C4 D
HWD kg 1.57E-07 9.36E-10 1.25E-10 0 1.04E-11 7.71E-11 3.99E-10 -6.45E-07
NHWD kg 1.75E+00 9.85E-04 8E-03 0 1.09E-05 5E-03 1.32E-01 -9.25E-01
RWD kg 4.95E-03 1.04E-05 4.45E-06 0 1.15E-07 7.51E-07 2.98E-07 -6E-03
CRU kg 0 0 0 0 0 0 0 0
MFR kg 0 0 0 0 0 1.65E+00 0 0
MER kg 0 0 0 0 0 0 0 0
EEE MJ 0 0 4.05E-01 0 0 0 0 0
EET MJ 0 0 7.35E-01 0 0 0 0 0
HWD = Hazardous waste disposed; NHWD = Non-hazardous waste disposed; RWD = Radioactive waste disposed; CRU = Components for re-use;
MFR = Materials for recycling; MER = Materials for energy recovery; EEE = Exported electrical energy; EET = Exported thermal energy
4 Environmental Product Declaration - dormakaba - ITS 915/ITS 900
RESULTS OF THE LCA – additional impact categories according to EN 15804+A2-optional:
1 door closer
Parameter Unit A1-A3 A4 A5 C1 C2 C3 C4 D
Disease
PM 8.72E-07 7.64E-08 4.16E-10 0 3.96E-11 9.91E-11 1.77E-10 -2.44E-07
incidence
IR kBq U235 eq 7.99E-01 1E-03 6.88E-04 0 1.64E-05 6.76E-05 3.07E-05 -1.2E+00
ETP-fw CTUe 4.26E+01 6.82E+00 4E-02 0 7.6E-02 8E-03 1.5E-02 -2.02E+01
HTP-c CTUh 6.25E-09 1.28E-10 2.12E-12 0 1.42E-12 6.57E-13 2.22E-12 -5.98E-10
HTP-nc CTUh 1.36E-07 5.58E-09 9.2E-11 0 6.08E-11 6.66E-11 2.44E-10 -7.65E-09
SQP SQP 4.67E+01 2.5E-02 2.2E-02 0 2.74E-04 6E-03 5E-03 -1.65E+00
PM = Potential incidence of disease due to PM emissions; IR = Potential Human exposure efficiency relative to U235; ETP-fw = Potential comparative
Toxic Unit for ecosystems; HTP-c = Potential comparative Toxic Unit for humans (cancerogenic); HTP-nc = Potential comparative Toxic Unit for humans
(not cancerogenic); SQP = Potential soil quality index
Disclaimer 1 – for the indicator “Potential Human exposure efficiency relative to U235”. This impact category deals mainly with the
eventual impact of low-dose ionizing radiation on human health of the nuclear fuel cycle. It does not consider effects due to possible
nuclear accidents, occupational exposure or radioactive waste disposal in underground facilities. Potential ionizing radiation from the
soil, radon and from some construction materials is also not measured by this indicator.
Disclaimer 2 – for the indicators “abiotic depletion potential for non-fossil resources”, “abiotic depletion potential for fossil resources”,
“water (user) deprivation potential, deprivation-weighted water consumption”, “potential comparative toxic unit for ecosystems”,
“potential comparative toxic unit for humans – cancerogenic”, “Potential comparative toxic unit for humans - not cancerogenic”,
“potential soil quality index”. The results of this environmental impact indicator shall be used with care as the uncertainties on these
results are high as there is limited experience with the indicator.
References
ECHA
European Chemicals Agency: https://echa.europa.eu/de/home GaBi
Sphera Solutions GmbH
DIN EN 1154:2003-04 Gabi Software System and Database for Life Cycle Engineering
Building hardware - Controlled door closing devices - 1992-2020 Version 10.0.0.71
Requirements and test methods University of Stuttgart Leinfelden-Echterdingen
EN15804 GaBi ts documentation
EN15804+A2:2019+AC:2021, Sustainability of construction GaBi life cycle inventory data documentation
works — Environmental Product Declarations — Core rules for (https://www.gabi-software.com/support/gabi/gabidatabase-
the product category of construction products 2020-lci-documentation/)
ISO 14025 LCA-tool dormakaba
DIN EN ISO 14025:201110, Environmental labels and LCA tool IBU-DOR-202104-LT1-EN, version 1.0, 2021.
declarations — Type III environmental declarations — Developed by Sphera Solutions GmbH
Principles and procedures
PCR Part A
REACH PCR – Part A: Calculation Rules for the Life Cycle Assessment
Registration, Evaluation, Authorisation and Restriction of and Requirements on the Project Re-port according to EN
Chemicals (REACH), Regulation (EC) No 1907/2006 15804+A2:2019, Version 1.0, 2020, Institut Bauen und Umwelt
e.V., www.ibu-epd.com
Further References
PCR Part B
cUL PCR – Part B: Requirements on the EPD for Building
Underwriters Laboratories Of Canada Hardware product, version 1.2, Institut Bauen und
Umwelt e.V., www.ibu-epd.com, 2017
IBU
Institut Bauen und Umwelt e.V.: General Programme
Instructions for the Preparation of EPDs at the Institut Bauen
und Umwelt e.V. Version 1., Berlin: Institut Bauen und Umwelt
e.V., 2016. www.ibu-epd.com
5 Environmental Product Declaration - dormakaba - ITS 915/ITS 900
Publisher
Institut Bauen und Umwelt e.V. +49 (0)30 3087748- 0
Hegelplatz 1 info@ibu-epd.com
10117 Berlin www.ibu-epd.com
Germany
Programme holder
Institut Bauen und Umwelt e.V. +49 (0)30 3087748- 0
Hegelplatz 1 info@ibu-epd.com
10117 Berlin www.ibu-epd.com
Germany
Author of the Life Cycle Assessment
Sphera Solutions GmbH +49 711 341817-0
Hauptstraße 111- 113 info@sphera.com
70771 Leinfelden-Echterdingen www.sphera.com
Germany
Owner of the Declaration
dormakaba International Holding GmbH +49 2333 793-0
DORMA Platz 1 info.de@dormakaba.com
58256 Ennepetal www.dormakaba.com
Germany
6 Environmental Product Declaration - dormakaba - ITS 915/ITS 900
