ENVIRONMENTAL PRODUCT DECLARATION
as per ISO 14025 and EN 15804+A2
Owner of the Declaration ARGE – The European Federation of Locks and Building Hardware Manufacturers
Publisher Institut Bauen und Umwelt e.V. (IBU)
Programme holder Institut Bauen und Umwelt e.V. (IBU)
Declaration number EPD-ARG-20230553-IBG1-EN
Issue date 02.04.2024
Valid to 01.04.2029
Push button locks
ARGE - The European Federation of Locks
and Building Hardware Manufacturers
This EPD is valid only for products supplied by an ARGE EPD licence holder.
www.ibu-epd.com | https://epd-online.com
1. General Information
ARGE - The European Federation of Locks Push button locks
and Building Hardware Manufacturers
Programme holder Owner of the declaration
IBU – Institut Bauen und Umwelt e.V. ARGE – The European Federation of Locks and Building Hardware
Hegelplatz 1 Manufacturers
10117 Berlin Offerstraße 12
Germany 42551 Velbert
Germany
Declaration number Declared product / declared unit
EPD-ARG-20230553-IBG1-EN 1 kg of push button lock
This declaration is based on the product category rules: Scope:
Building Hardware products, 01.08.2021 This ARGE EPD covers mechanically operated push button locks, used to
(PCR checked and approved by the SVR) secure openings by purely mechanical means (i.e., no
electrics/electronics). The reference product selected to calculate the
impact this group of products has on the environment is a push button lock
Issue date composed primarily of Zamak and steel. This product is the only one
assessed for this EPD and serves as a reference to cover all products of
02.04.2024
ARGE member companies within this group. In agreement with ARGE it
has been determined to be the most representative product of this group,
based on its market share.
Valid to
The owner of the declaration shall be liable for the underlying information
01.04.2029 and evidence; the IBU shall not be liable with respect to manufacturer
information, life cycle assessment data and evidences.
The EPD was created according to the specifications of EN 15804+A2. In
the following, the standard will be simplified as EN 15804.
Verification
The standard EN 15804 serves as the core PCR
Independent verification of the declaration and data according to ISO
14025:2011
internally X externally
Dipl.-Ing. Hans Peters
(Chairman of Institut Bauen und Umwelt e.V.)
Florian Pronold Dr. Matthew Fishwick,
(Managing Director Institut Bauen und Umwelt e.V.) (Independent verifier)
1 Environmental Product Declaration - ARGE - The European Federation of Locks and Building Hardware Manufacturers - Push button locks
2. Product
formed by injection moulding or other thermal forming
2.1 Product description/Product definition
processes.
This EPD covers mechanically operated push button locksets
and their locking plates for the use on doors, window doors and Nylon 66 is a polymer, in particular polyamide. It is formed by
entrance doors in buildings to keep them in the closed position the polycondensation of hexamethylenediamine and adipic acid
until the correct combination of buttons is entered. in equal parts. Components made of Nylon 66 are formed by
injection moulding or other thermal forming processes.
For the application and use the respective national provisions
apply. 1) This product/article/at least one partial article contains
substances listed in the ECHA candidate list (date: 14.06.2023)
2.2 Application
exceeding 0.1 percentage by mass: Certain components may
These products are designed to be integrated into door contain small amounts of lead (CAS no. 7439-92-1) as an
assemblies consisting of various materials and used for various alloying element.
applications. They can be used for either interior or exterior
doors as well as for gates, following the instructions of the
2) This product/article/at least one partial article contains other
manufacturer.
cancerogenic, mutagenic, reprotoxic (CMR) substances in
categories 1A or 1B which are not on the ECHA candidate list,
2.3 Technical Data
exceeding 0.1 percentage by mass: no.
No classes are defined as no EN standard exists. Performance
data of the product with respect to its characteristics in
3) Biocide products were added to this construction product or it
accordance with the relevant technical provision (no CE-
has been treated with biocide products (this then concerns a
marking).
treated product as defined by the (EU) Ordinance on Biocide
Products No. 528/2012): no.
2.4 Delivery status
The products are sold by unit. Deliveries of individual items are 2.6 Manufacture
possible but are an exception. Standard deliveries comprise a
The manufacture of a push button lock usually follows a 3-step
larger quantity of locks, as they are marketed as "B2B"
process:
products and not to end-users.
1. Manufacture of components: this step might include a
2.5 Base materials/Ancillary materials surface treatment in the factory or by external
The base materials of the product analysed for this EPD are contractors.
shown in the following table: 2. Pre-assembly of modules (in the factory).
3. Final assembly (in the factory).
Name Value Unit
Zamak 78.24 % 2.7 Environment and health during manufacturing
Steel 9.87 % Regular measurements of air quality and noise levels are
Stainless steel 9.6 % carried out by the manufacturers, the ARGE member
Brass 1.79 % companies. The results shall be within the mandatory safety
levels. In areas where employees are exposed to chemical
Sintered iron 0.44 %
products, the required protective clothing and technical
Acrylic 0.000269 %
protective devices shall be provided. Regular health checks are
Nylon 66 0.000179 % mandatory for employees in production facilities.
Zamak is an alloy with a base metal of zinc and alloying
2.8 Product processing/Installation
elements of aluminium, magnesium, and copper. Components
The installation of the product may vary depending on the type
made from Zamak are die-cast.
of door or gate and the specific situation, but the products shall
not require energy consumption for installation.
Steel is produced by combining iron with carbon as well as
other elements depending on the desired characteristics.
2.9 Packaging
Components made of steel are formed by stamping or other
Normally, each individual product is packed in paper or
types of mechanical processing.
cardboard. These individual products are then packed in a
cardboard box and stacked on wooden pallets for transport to
Stainless steel is produced by combining iron with chromium
the customer.
as well as other elements depending on the desired
characteristics. Components made of steel are formed by
Waste from product packaging is collected separately for waste
stamping or other types of mechanical processing.
disposal (including recycling).
Brass is an alloy of zinc and copper. Components made of 2.10 Condition of use
brass are made by forging, die-casting or other types of
Once installed, the products shall require no servicing during
mechanical processing.
their expected service lives. There shall be no consumption of
water or energy linked to their use, and they shall not cause
Sintered iron is produced by a process in which powdered any emissions.
metal is pressed into a specific shape and then heated to bond
the metal particles in the designed shape of the component. 2.11 Environment and health during use
No environmental damage or health risks are to be expected
Acrylic, used in resin form, is a thermoplastic or thermosetting during normal conditions of use.
plastic substance typically derived from acrylic acid, methacrylic
acid and acrylate monomers. Components made of Acrylic are 2.12 Reference service life
2 Environmental Product Declaration - ARGE - The European Federation of Locks and Building Hardware Manufacturers - Push button locks
The reference service life is 30 years under normal working In case of mechanical destruction of the declared product, it
conditions. This corresponds to passing a mechanical does not perform any impact on the environment or alter its
endurance test of 100.000 cycles as specified in the British substantial composition.
Standard BS 8607. The reference service life is dependent on
the actual frequency of use and environmental conditions. It is 2.14 Re-use phase
required that installation, as well as maintenance of the Removal of push button locks (for re-use or recycling) shall
product, must be done in line with instructions provided by the have no adverse effect on the environment.
manufacturer.
2.15 Disposal
2.13 Extraordinary effects Push button locks should be re-cycled wherever possible,
Fire providing that there is no adverse effect on the environment
There are no specific fire resistance requirements. The waste code in accordance with the European Waste Code
is 17 04 07.
Water
2.16 Further information
The declared product is intended to be used in and around
buildings under normal conditions (indoor or outdoor use). It Details of all types and variants can be found on the
shall not emit hazardous substances in the event of flooding. manufacturers' websites. The respective website addresses are
available at https://arge.org.
Mechanical destruction
3. LCA: Calculation rules
account (corresponding to the process 'Grinding,
3.1 Declared Unit metals'). Only then, is the material considered to have
The declared unit for all products covered by ARGE EPD is 1 attained the 'end-of-waste' state.
kg (of product). Since individual products will rarely weigh • each type of waste is modelled as a transport to the
exactly 1kg it is necessary to establish the exact weight of the treatment site with a distance of 30 km. Parts sent for
product and then use this as a correction factor to determine recycling include electricity consumption (grinding) and
the true values for 1 kg of product in the tables (Section 5). a flow ('Materials for recycling, unspecified').
Declared unit
3.3 Estimates and assumptions
Name Value Unit
The LCA data of the declared push button lock had been
Declared unit 1 kg calculated by the production data from a total of one ARGE
Mass of declared product 1.115 kg member company. This company had been chosen by ARGE
Raw density 1 kg/m3 as being representative by means of its production processes
and its market share. The product is chosen to be as
representative as possible.
3.2 System boundary 3.4 Cut-off criteria
Type of the EPD: "cradle to gate with options, with modules C1 The cut-off criteria considered are 1% of renewable and non-
– C4, and module D (A1-A3, C1-C3, D and additional renewable primary energy usage and 1% of the total mass of
modules)" that unit process. The total neglected input flows per module
shall be a maximum of 5% of energy usage and mass.
The analysis of the product life cycle includes the production
and transport of the raw materials, the manufacture of the For this study, all input and output flows have been considered
product and the packaging materials which are declared in at 100%, including raw materials as per the product
modules A1-A3. composition provided by the manufacturer and packaging of
Losses during production are considered as waste and are sent raw materials as well as the final product. Energy and water
for recycling. No recycling processes are taken into account consumptions have also been considered at 100% according to
except for transport and electricity consumption for grinding the the data provided.
metals. When recycled metals are used as raw material only
their transformation process is taken into account and not the With the approach chosen, no significant environmental
extraction of the raw material. impacts are known to have been cut off.
A4 module represents the transport of the finished push button
lock to the installation site. 3.5 Background data
There is no waste associated with the installation of the For the life cycle modelling of the considered product, all
product. The A5 module therefore represents only the disposal relevant background datasets are taken from ecoinvent v3.8
of the product packaging. (system model: cut-off by classification).
The End-of-Life (EoL) stages are also considered. The
transportation to the EoL disposal site is taken into account in 3.6 Data quality
module C2. Module C4 covers the disposal of the locks. Module The objective of this evaluation is to evaluate the environmental
C3 covers the recycling of the individual elements according to impacts generated by the products throughout their entire life
European averages, with the remaining waste divided between cycles. To this end, ISO 14040, ISO 14044 and EN 15804 have
incineration and landfill. Such a mixed scenario is declared due been met regarding the quality of data on the following different
to the complex material mix of the product and the dependency criteria:
of the EoL-route on the EoL-route of the product the push
button lock has been integrated into. Time: The life cycle inventory data used come from:
In practice, the end of life has been modelled as follows:
• Data collected specifically for this study on the ARGE
• when a material is sent for recycling, generic transport member company's manufacturing site. Datasets are
and electric consumption of a shredder is taken into based on 1-year averaged data (time period: January
3 Environmental Product Declaration - ARGE - The European Federation of Locks and Building Hardware Manufacturers - Push button locks
2013 to December 2013 considered representative for Land or region, in which the declared product system is
2022). manufactured, used or handled at the end of the product´s
• In the absence of collected data, generic data from the lifespan: Europe
ecoinvent v3.8 database have been used. This is
updated regularly and is representative of current
processes (the entire database having been updated in 3.9 Allocation
2021). The products covered by this EPD are produced in numerous
Geography: Data on the composition of products, process sites. The product assessed for the calculation of this EPD is
technologies, wastage, etc. come from the production site of produced by one manufacturer on one site. All data were
the ARGE member company. Generic data on processing provided by this manufacturer of the products per unit, and then
processes come from the ecoinvent database, representative divided by the mass of the product to give a value per kg of
for European production processes. product produced.
Technology: Material shaping technologies are based on The assumptions relating to the EoL of the product are
European technology in the case of the use of generic data. described in the section System Boundaries.
3.10 Comparability
In this EPD, a representative product has been selected to
represent the product group, considering the most common Basically, a comparison or an evaluation of EPD data is only
materialisation of the products covered in this product group. possible if all the data sets to be compared were created
according to EN 15804 and the building context, respectively
3.7 Period under review the product-specific characteristics of performance, are taken
The data of the LCA is based on the annual production data of into account.
an ARGE member from 2013, considered representative for the
year 2022. ecoinvent v3.8 (system model: cut-off by classification) has
been used as the background database.
3.8 Geographic Representativeness
4. LCA: Scenarios and additional technical information
It is assumed that a 16–32-ton truck is used to transport the
Characteristic product properties of biogenic carbon
product:
- Transport to shredding facility for metal recovery: 150 km
Information on the biogenic carbon content at factory gate - Transport to municipal waste incineration plant: 50 km
- Transport to landfill: 30 km
Note: 1 kg of biogenic carbon is equivalent to 44/12 kg of CO .
2
Name Value Unit Reuse, recovery and/or recycling potentials (D), relevant
kg scenario information
Biogenic carbon content in product 0
C
Biogenic carbon content in accompanying kg Module D contains the benefits and loads beyond the system
0.0362
packaging C boundary related to the recycling of metals, which result from
the treatment of recycled materials from the point of end-of-
waste status to the point of substitution (as costs) and the
The following information is the basis of the declared modules
substitution of primary resources (as benefits).
within the LCA in this EPD.
Transport to the building site (A4) According to EN 16710, clause 6.4.3.3: 'In module D
Name Value Unit substitution effects are calculated only for the resulting net
output flow.
Litres of fuel 25.8 l/100km
Transport distance 3500 km
For building hardware, the following rules apply for the
Capacity utilisation (including empty runs) 36 % quantification of net output flows:
- all production scrap and cuttings leave modules A1-B3 as
Installation into the building (A5)
sorted scrap without allocated burdens from primary production;
Name Value Unit the corresponding amounts are declared as material for
Material loss 0.0949 kg recycling (MFR);
- net amounts of a metal leaving the product system are
quantified as the material for recycling leaving modules A1-C4
Reference service life minus the input of secondary scrap (secondary material, SM) to
Name Value Unit the product system;
- in the case of brass and zinc alloys, which are composed of
Reference service life 30 a
two different constituting metals, no difference shall be made
Test cycles over RSL (BS 8607) 100'000 cycles
between the input of secondary constituting metals (Cu and Zn;
Cu and Sn) and its alloys (CuZn; CuSn).
End of life (C1-C4)
Name Value Unit
Negative net output flows shall not be considered in the
Collected separately waste type 1 kg quantification of module D.'
Recycling 0.241 kg
Energy recovery 0.349 kg It also includes the benefits and loads related to 'exported
energy electricity' and 'exported energy heat' resulting from the
Landfilling 0.41 kg
energy recovery from plastic wastes in a municipal waste
incineration plant as modelled in Modules A3, A5 and C4.
4 Environmental Product Declaration - ARGE - The European Federation of Locks and Building Hardware Manufacturers - Push button locks
5. LCA: Results
In Table 1 "Description of the system boundary", the declared modules are indicated with an "X"; all modules that are not declared
within the EPD but where additional data are available are indicated with "MND". Those data can also be used for building assessment
scenarios. The values are declared with three valid digits in exponential form.The set of characterisation factors EF3.0 has been used
for the life cycle assessment.
DESCRIPTION OF THE SYSTEM BOUNDARY (X = INCLUDED IN LCA; MND = MODULE OR INDICATOR NOT DECLARED; MNR
= MODULE NOT RELEVANT)
Benefits and
Construction loads beyond
Product stage Use stage End of life stage
process stage the system
boundaries
la ire wta am R y lp p u s tro p s n a rT g n iru tc a fu n a M tro p s nm ae o rh r
T
f te tis e h t o t e ta g y lb m e s s A e s U e c n a n e tn ia M ria p e R tn e m e c a lp e R tn e m h s ib ru fe R la n o ity ag rr ee pn Oe e s u la n o ita r re et pa Ow e s u n o itc u rts n eo Dc -n o itilo m e d tro p s n a rT g n is s ee tsc ao Wrp la s o p s iD e s u e R- y re v o c e R- g n ilc y c e R- la itn e to p
A1 A2 A3 A4 A5 B1 B2 B3 B4 B5 B6 B7 C1 C2 C3 C4 D
X X X X X MND MND MNR MNR MNR MND MND X X X X X
RESULTS OF THE LCA - ENVIRONMENTAL IMPACT according to EN 15804+A2: 1 kg of push button lock
Parameter Unit A1-A3 A4 A5 C1 C2 C3 C4 D
GWP-total kg CO2 eq 5.38E+00 6.24E-01 1.59E-01 0 1.43E-02 2.99E-03 4.69E-03 -1.81E+00
GWP-fossil kg CO2 eq 5.49E+00 6.24E-01 2.65E-02 0 1.43E-02 2.99E-03 4.69E-03 -1.81E+00
GWP-biogenic kg CO2 eq -1.33E-01 0 1.33E-01 0 0 0 0 0
GWP-luluc kg CO2 eq 1.47E-02 2.5E-04 7.63E-07 0 5.74E-06 7.45E-06 3.38E-06 -5.32E-03
ODP kg CFC11 eq 2.9E-07 1.45E-07 4.11E-10 0 3.32E-09 1.51E-10 1.16E-09 -7.14E-08
AP mol H+ eq 6.28E-02 1.77E-03 1.43E-05 0 4.07E-05 1.54E-05 2.95E-05 -2.14E-02
EP-freshwater kg P eq 3.78E-04 4.45E-06 2.12E-08 0 1.02E-07 3.36E-07 6.41E-08 -1.26E-04
EP-marine kg N eq 6.65E-03 3.52E-04 5.69E-06 0 8.09E-06 1.97E-06 9.83E-06 -2.19E-03
EP-terrestrial mol N eq 7.6E-02 3.93E-03 6.12E-05 0 9.02E-05 2.28E-05 1.08E-04 -2.52E-02
kg NMVOC
POCP 2.24E-02 1.51E-03 1.62E-05 0 3.47E-05 6.23E-06 3.32E-05 -7.33E-03
eq
ADPE kg Sb eq 1.83E-03 2.21E-06 7.13E-09 0 5.08E-08 7.24E-09 1.29E-08 -7.41E-04
ADPF MJ 6.09E+01 9.46E+00 2.95E-02 0 2.17E-01 6.33E-02 8.72E-02 -1.93E+01
m3 world eq
WDP 1.71E+00 2.88E-02 2.59E-04 0 6.62E-04 7.07E-04 -1.13E-03 -5.79E-01
deprived
GWP = Global warming potential; ODP = Depletion potential of the stratospheric ozone layer; AP = Acidification potential of land and water; EP =
Eutrophication potential; POCP = Formation potential of tropospheric ozone photochemical oxidants; ADPE = Abiotic depletion potential for non-fossil
resources; ADPF = Abiotic depletion potential for fossil resources; WDP = Water (user) deprivation potential)
RESULTS OF THE LCA - INDICATORS TO DESCRIBE RESOURCE USE according to EN 15804+A2: 1 kg of push button lock
Parameter Unit A1-A3 A4 A5 C1 C2 C3 C4 D
PERE MJ 7.93E+00 1.33E-01 -7.09E-01 0 3.06E-03 1.2E-02 1.26E-03 -2.64E+00
PERM MJ 1.24E+00 0 3.32E-01 0 0 0 0 0
PERT MJ 9.17E+00 1.33E-01 -3.77E-01 0 3.06E-03 1.2E-02 1.26E-03 -2.64E+00
PENRE MJ 6.07E+01 9.47E+00 3.84E-01 0 2.18E-01 6.39E-02 9.32E-02 -1.93E+01
PENRM MJ 3.68E-01 0 -3.55E-01 0 0 0 -5.96E-03 0
PENRT MJ 6.11E+01 9.47E+00 2.95E-02 0 2.18E-01 6.39E-02 8.72E-02 -1.93E+01
SM kg 1.1E-01 0 0 0 0 0 0 0
RSF MJ 0 0 0 0 0 0 0 0
NRSF MJ 0 0 0 0 0 0 0 0
FW m3 5.59E-02 1E-03 5.29E-05 0 2.31E-05 4.08E-05 2.19E-04 -1.95E-02
PERE = Use of renewable primary energy excluding renewable primary energy resources used as raw materials; PERM = Use of renewable primary
energy resources used as raw materials; PERT = Total use of renewable primary energy resources; PENRE = Use of non-renewable primary energy
excluding non-renewable primary energy resources used as raw materials; PENRM = Use of non-renewable primary energy resources used as raw
materials; PENRT = Total use of non-renewable primary energy resources; SM = Use of secondary material; RSF = Use of renewable secondary fuels;
NRSF = Use of non-renewable secondary fuels; FW = Use of net fresh water
RESULTS OF THE LCA – WASTE CATEGORIES AND OUTPUT FLOWS according to EN 15804+A2:
1 kg of push button lock
Parameter Unit A1-A3 A4 A5 C1 C2 C3 C4 D
HWD kg 2.36E-04 2.47E-05 1.71E-07 0 5.68E-07 2.24E-08 1.67E-07 -6.99E-05
NHWD kg 1.9E+00 4.98E-01 2.28E-03 0 1.14E-02 2.38E-04 3.81E-01 -3.55E-01
RWD kg 2.92E-04 1.37E-04 3.49E-07 0 3.15E-06 8.51E-07 1.12E-06 -6.93E-05
CRU kg 0 0 0 0 0 0 0 0
MFR kg 1.26E-02 0 4.22E-02 0 0 4.47E-01 0 0
MER kg 0 0 0 0 0 0 0 0
5 Environmental Product Declaration - ARGE - The European Federation of Locks and Building Hardware Manufacturers - Push button locks
EEE MJ 0 0 3.98E-02 0 0 0 2.53E-04 0
EET MJ 0 0 2.64E-01 0 0 0 1.67E-03 0
HWD = Hazardous waste disposed; NHWD = Non-hazardous waste disposed; RWD = Radioactive waste disposed; CRU = Components for re-use;
MFR = Materials for recycling; MER = Materials for energy recovery; EEE = Exported electrical energy; EET = Exported thermal energy
RESULTS OF THE LCA – additional impact categories according to EN 15804+A2-optional:
1 kg of push button lock
Parameter Unit A1-A3 A4 A5 C1 C2 C3 C4 D
Disease
PM 4.44E-07 5.01E-08 2.03E-10 0 1.15E-09 4.11E-11 9.32E-10 -1.33E-07
incidence
IR kBq U235 eq 1.45E-01 4.11E-02 1.08E-04 0 9.44E-04 5.76E-04 3.35E-04 -3.9E-02
ETP-fw CTUe 5.16E+02 7.43E+00 3.12E-02 0 1.71E-01 3.18E-02 1.57E-01 -1.82E+02
HTP-c CTUh 3.43E-08 2.39E-10 3.06E-12 0 5.49E-12 8.51E-13 8.98E-12 -1.04E-08
HTP-nc CTUh 1.15E-06 7.5E-09 1.28E-10 0 1.72E-10 2.76E-11 8.45E-11 -4.26E-07
SQP SQP 4.49E+01 6.6E+00 1.74E-02 0 1.52E-01 9.73E-03 1.5E-01 -1.1E+01
PM = Potential incidence of disease due to PM emissions; IR = Potential Human exposure efficiency relative to U235; ETP-fw = Potential comparative
Toxic Unit for ecosystems; HTP-c = Potential comparative Toxic Unit for humans (cancerogenic); HTP-nc = Potential comparative Toxic Unit for humans
(not cancerogenic); SQP = Potential soil quality index
Disclaimer 1 – for the indicator 'Potential Human exposure efficiency relative to U235'. This impact category deals mainly with the
eventual impact of low-dose ionizing radiation on human health of the nuclear fuel cycle. It does not consider effects due to possible
nuclear accidents, occupational exposure or radioactive waste disposal in underground facilities. Potential ionizing radiation from the
soil, radon and from some construction materials is also not measured by this indicator.
Disclaimer 2 – for the indicators 'abiotic depletion potential for non-fossil resources', 'abiotic depletion potential for fossil resources',
'water (user) deprivation potential, deprivation-weighted water consumption', 'potential comparative toxic unit for ecosystems', 'potential
comparative toxic unit for humans – cancerogenic', 'Potential comparative toxic unit for humans - not cancerogenic', 'potential soil
quality index'. The results of this environmental impact indicator shall be used with care as the uncertainties on these results are high
as there is limited experience with the indicator.
6. LCA: Interpretation
Figure 1 illustrates the relative contributions of the different
modules along the life cycle of the declared product.
Figure 1: Environmental impacts of push button locks Benefits and burdens beyond the system boundary (module D)
along its life cycle are in the order of 20% to 30% of the impacts over the product
life cycle (modules A1-A3) and relate basically to the recycling
The largest part of environmental impacts is caused during of metals.
production (modules A1-A3); comparably small impacts are In this EPD, a representative product has been selected to
caused during the transport of the product to the construction represent the product group, considering the most common
site (via the manufacturer of the product, which the push button materialisation of the products covered in this product group.
lock has been integrated into). This has been done based on the knowledge of ARGE
members on the composition of the declared products. In in-
All the other modules related to the product life cycle are not depth analysis of variability has not been conducted for this
significant. product group.
6 Environmental Product Declaration - ARGE - The European Federation of Locks and Building Hardware Manufacturers - Push button locks
7. Requisite evidence
No testing results are required by the PCR part B.
8. References
Product category rules of IBU
BS 8607
IBU (2021) BS 8607:2014+A1:2016, Mechanically operated push-button
IBU (2021): General Instructions for the EPD Programme of the locksets. Requirements and test methods.
Institut Bauen und Umwelt e.V. (General Instructions for the
IBU EPD Programme). Version 2.0, Institut Bauen und Umwelt, ISO 15686
Berlin. ISO 15686:1, -2, -7 and -8. Service life planning (various parts).
IBU (2021) ECHA candidate list
IBU (2021): PCR Part A: Calculation rules for the life cycle Candidate List of substances of very high concern for
assessment and requirements on the project report according Authorisation, published in accordance with Article 59(10) of the
to EN 15804+A2. Version 1.3., Institut Bauen und Umwelt, REACH Regulation. European Chemicals Agency, Brussels.
Berlin.
Ordinance on Biocide Products No. 528/2012
IBU (2023) REGULATION (EU) No 528/2012 OF THE EUROPEAN
IBU (2023): PCR Part B: Requirements on the EPD for building PARLIAMENT AND OF THE COUNCIL of 22 May 2012
hardware products. Version 2023/04, Institut Bauen und concerning the making available on the market and use of
Umwelt, Berlin. biocidal products.
Standards and legal documents European List of Waste
Commission Decision of 3 May 2000 replacing Decision
EN 15804 94/3/EC establishing a list of wastes pursuant to Article 1(a) of
EN 15804:2012+A2:2019+AC:2021, Sustainability of Council Directive 75/442/EEC on waste and Council Decision
construction works - Environmental product declarations - Core 94/904/EC establishing a list of hazardous waste pursuant to
rules for the product category of construction products. Article 1(4) of Council Directive 91/689/EEC on hazardous
waste (notified under document number C(2000) 1147).
EN 17610
EN 17610:2022, Building hardware - Environmental product Additional references
declarations - Product category rules complementary to EN
15804 for building hardware. BBSR 2017
BBSR (2017): Nutzungsdauer von Bauteilen in
ISO 14025 Lebenszyklusanalysen nach Bewertungssystem Nachhaltiges
ISO 14025:2006-07, Environmental labels and declarations - Bauen (BNB). Version vom 24.10.2017, Bundesinstitut für Bau-,
Type III Environmental declarations - Principles and Stadt- und Raumforschung, Berlin.
procedures.
ecoinvent v3.8
ISO 14044 https://www.ecoinvent.org
EN ISO 14044:2006-07, Environmental management - Life
cycle assessment - Requirements and guidance (ISO
14044:2006).
7 Environmental Product Declaration - ARGE - The European Federation of Locks and Building Hardware Manufacturers - Push button locks
Publisher
Institut Bauen und Umwelt e.V. +49 (0)30 3087748- 0
Hegelplatz 1 info@ibu-epd.com
10117 Berlin www.ibu-epd.com
Germany
Programme holder
Institut Bauen und Umwelt e.V. +49 (0)30 3087748- 0
Hegelplatz 1 info@ibu-epd.com
10117 Berlin www.ibu-epd.com
Germany
Author of the Life Cycle Assessment
Dr. Frank Werner - Umwelt & Entwicklung + 41 (0)44 241 39 06
Kammelenbergstrasse 30 frank@frankwerner.ch
9011 St. Gallen http://www.frankwerner.ch/
Switzerland
Owner of the Declaration
ARGE – The European Federation of Locks and +49 (0)2051 9506 15
Building Hardware Manufacturers mail@arge.org
Offerstraße 12 www.arge.org
42551 Velbert
Germany
8 Environmental Product Declaration - ARGE - The European Federation of Locks and Building Hardware Manufacturers - Push button locks
