ENVIRONMENTAL PRODUCT DECLARATION
as per ISO 14025 and EN 15804+A2
Owner of the Declaration VdL - Verband der deutschen Lack- und Druckfarbenindustrie e.V.
Publisher Institut Bauen und Umwelt e.V. (IBU)
Programme holder Institut Bauen und Umwelt e.V. (IBU)
Declaration number EPD-VDL-20230163-IAG1-EN
Issue date 22/06/2023
Valid to 21/06/2028
Polyester Powder Coating
Verband der deutschen Lack- und
Druckfarbenindustrie e.V.
www.ibu-epd.com | https://epd-online.com
1. General Information
Verband der deutschen Lack- und Polyester Powder Coating
Druckfarbenindustrie e.V.
Programme holder Owner of the declaration
IBU – Institut Bauen und Umwelt e.V. VdL - Verband der deutschen Lack- und Druckfarbenindustrie e.V.
Hegelplatz 1 Mainzer Landstraße 55
10117 Berlin 60329 Frankfurt a. M.
Germany Germany
Declaration number Declared product / declared unit
EPD-VDL-20230163-IAG1-EN 1 kg polyester-based powder coating
This declaration is based on the product category rules: Scope:
Coatings with organic binders, 01/08/2021 This association EPD applies to a specific polyester-based powder coating
(PCR checked and approved by the SVR) customary in the industry of the member companies of the Verband der
deutschen Lack- und Druckfarbenindustrie e.V. (VdL). All the companies of
the VdL's powder coatings specialist group mentioned in section 8
Issue date participated in the preparation of the Life Cycle Assessment for this
association EPD. In terms of number, they represent 100% of the powder
22/06/2023
coatings manufacturers in the VdL.
The declared formulation describes an industry-standard powder coating
with corresponding pigment and titanium dioxide contents as listed in
Valid to
section 2.5. The data relating to the declared unit results from the survey of
21/06/2028 powder coating manufacturers in the VdL. The members of the VdL are
primarily based in Germany which is why Germany was used as a
geographic reference in the EPD. Two of the manufacturing companies
have their production facilities in Austria and Switzerland, respectively. The
validity of this EPD for Austrian and Swiss production is outlined in section
3.3.
This document is translated from the German Environmental Product
Declaration into English. It is based on the German original version EPD-
VDL-20230163-IAG1-DE. The verifier has no influence on the quality of the
translation.
The owner of the declaration shall be liable for the underlying information
and evidence; the IBU shall not be liable with respect to manufacturer
Dipl.-Ing. Hans Peters
information, life cycle assessment data and evidences.
(Chairman of Institut Bauen und Umwelt e.V.)
The EPD was created according to the specifications of EN 15804+A2. In
the following, the standard will be simplified as EN 15804.
Verification
The standard EN 15804 serves as the core PCR
Independent verification of the declaration and data according to ISO
14025:2011
internally X externally
Florian Pronold Matthias Schulz,
(Managing Director Institut Bauen und Umwelt e.V.) (Independent verifier)
1 Environmental Product Declaration - Verband der deutschen Lack- und Druckfarbenindustrie e.V. - Polyester Powder Coating
2. Product
characteristics according to the applicable technical regulation
2.1 Product description/Product definition (no CE marking).
This Environmental Product Declaration declares a specific
polyester powder coating that is customary in the industry and 2.4 Delivery status
is produced by the powder coating manufacturers (DACH The powder coating under review is supplied as ground
region) organised in the Verband der deutschen Lack- und powder. The powder coating is either packed in cardboard
Druckfarbenindustrie e.V. (VdL). The formulation was boxes lined with polyethylene (PE) bags (contents 15–25 kg), in
determined on the basis of a survey of the powder coating cardboard containers with 20–25 bags (contents 400–500 kg)
manufacturers in the VdL. or in Big Bags (contents 400–700 kg). Other containers are
The powder coating under review is an organic-based, available on request. The various containers are generally
thermally-hardening, duroplastic coating material which transported on wooden pallets which can be reused. The
complies with the state of the art. The powder coating materials used for packaging and transport should be recycled
comprises polyester resin with the corresponding curing agent, or thermally utilised where possible.
additives, suitable filler and weather-resistant pigments. The
use of the product is subject to the respective national 2.5 Base materials/Ancillary materials
regulations at the place of use, in Germany for example the
building regulations of the federal states, and the technical Name Value Unit
regulations based on these regulations.
Binding agents (resins and hardeners) 70 %
2.2 Application Pigments (coloured and effect pigments) 3 %
The polyester powder coating under review here satisfies the Titanium dioxide 15 %
requirements concerning weathering stability and therefore Extenders 10 %
offers long-term protection in outdoor applications. This powder Additives 2 %
coating is primarily used for coating aluminium and steel for
construction purposes in accordance with EN 12206-1 and the
The Declaration refers to the above composition of powder
specifications of the relevant quality associations, i.e. wherever
coating.
attractive durable colours are required. In the construction
sector, it can be primarily found in the area of bulk coatings for
1) The product contains substances on the ECHA Candidate
facade elements, window frames and doors.
List of 10.06.2022 of Substances of Very High Concern (SVHC)
2.3 Technical Data for authorisation above 0.1% by mass: no.
The powder coating film described and applied in accordance
with the specifications of the applicable technical data sheet 2) The product contains other CMR substances of category 1A
(coating thickness, curing conditions) displays the following or 1B, which are not on the ECHA Candidate List of
technical properties: 10.06.2022, above 0.1% by mass in at least one sub-product:
no.
Name Value Unit
3) Biocidal products have been added to the present building
Density ISO 8130-2 1.2 - 1.7 kg/m3
product or it has been treated with biocidal products (it is thus a
Solids content ISO 3251 100 % treated product within the meaning of the Biocidal Products
GU Regulation): no.
Gloss measuring angle 60° ISO
20 - 90 (Gloss
2813* Unit) 2.6 Manufacture
Manufacturing a powder coating involves the following
Salt spray resistance NSS, ISO >= 240 h,
- processing steps:
9227* dmax 2 mm
Water condensation test in constant >= 240 h, no • Weighing of the raw materials
-
atmospheres ISO 6270-1* bubbles • Mechanical premixing
• Melt homogenisation in the extruder
Permissible change in gloss. as per >= 200 h; > 50
• Rolling, cooling and crushing of the extrudate into chips
GSB/Qualicoat, accelerated % residual %
• Grinding and sieving
weathering ISO 16474-3* gloss
• Packaging and labelling.
Curing time (powder coatings) 5 - 20 min
Curing temperature 160 - 200 °C
Theoretical spreading rate in
accordance to the layer thickness (60 10 - 14 m2/kg
μm)
Hardness test ISO 1520* >= 2 mm
Mandrel bending test ISO 1519* <= 10 mm
* refers to the applied and cured powder coating film on the
suitable substrate
Other technical data in accordance with the PCR: Coatings with
organic binding agents are not of relevance for the declared
product.
2.7 Environment and health during manufacturing
Performance values of the product in relation to its
2 Environmental Product Declaration - Verband der deutschen Lack- und Druckfarbenindustrie e.V. - Polyester Powder Coating
In order to ensure protection of the environment and health, the
following environmental management systems and legal 2.9 Packaging
specifications are considered within the framework of the The powder coating under review is usually packed in
manufacturing process. cardboard containers lined with PE bags or in Big Bags. The
Typical environmental management systems (specific details various containers are generally transported on wooden pallets
can be requested from the respective manufacturer): which can be reused. The materials used for packaging and
transport should be recycled or thermally utilised where
• ISO 14004: General guidelines on principles, systems
possible.
and supporting the techniques
• ISO 14001: International standard for specifying and 2.10 Condition of use
implementing environmental requirements
In buildings, powder coatings are used as coatings on facades,
• EMAS Regulation and EC Eco-Audit Regulation:
metallic surfaces or similar. Powder-coated surfaces display a
voluntary participation of organisations in a Community
stable and constant composition during use. The decorative
eco-management and audit scheme.
and practical properties displayed by powder coatings in interior
or exterior applications permit a long service life on the part of
As the manufacturing process does not include solvents, no
the coated objects.
foul air emissions are incurred.
2.11 Environment and health during use
Dust emissions are prevented by state-of-the-art filter When powder coatings are processed as designated by the
technology. manufacturer and taking consideration of the applicable safety
information, no negative impacts are to be anticipated for man
The water used for cleaning the plants is cleaned and, where or the environment in accordance with the current state of
possible, redirected to the water cycle. knowledge.
No soil contamination occurs. 2.12 Reference service life
When processed as designated and taking consideration of the
Storage and handling of the raw materials, intermediates and information supplied by the manufacturer (cleaning
finished products takes consideration of statutory guidelines. recommendations, potential restrictions concerning areas of
application), the service life of powder-coated surfaces
Noise-generating aggregates are exclusively used in noise- complies with the service life of the coated parts.
insulating form with the result that the national limit values are
maintained or fallen short of.
2.13 Extraordinary effects
Reducing energy requirements per manufacturing unit is Fire
permanently pursued within the framework of an environmental In line with EN 13501-1, powder-coated construction products
or energy management system. are 'non-homogenous construction products'. The powder
coating and/or coating manufactured is defined as a 'non-
The use of substances classified as hazardous is avoided as substantial component' of the construction product. Reaction to
far as technically possible. If the use of hazardous substances fire must be examined individually and classified in a fire class
is technically necessary, it is ensured that the maximum by the manufacturer of the manufactured product.
occupational limit values are fallen short of and all statutory
protective measures are taken into consideration. Water
Marking associated with hazardous substances is regulated by When the powder coating is processed as designated, a hazard
CLP Regulation. The handling of hazardous substances is to water is not to be anticipated in accordance with the current
regulated by occupational health and safety regulations. state of knowledge in the event of unforeseen contact with
water.
As a general rule, the principle of avoidance, reduction and
legally-compliant disposal applies for waste. Mechanical destruction
In terms of mechanical destruction, powder coatings comply
The relevant legal specifications governing fire safety and with the requirement profile of the coated parts. Negative
explosion protection are maintained. impact on the environment in the event of unforeseen
mechanical destruction is not to be anticipated.
All employees are trained at regular intervals on the contents of
2.14 Re-use phase
the items listed above.
Material reuse of hardened powder coatings is not possible.
2.8 Product processing/Installation Powder coatings can be removed using mechanical, chemical
In its corresponding formulation, the powder coating under and thermal processes. Powder coatings removed by
review can be processed on all coating systems available on mechanical or chemical processes can then be directed to
the market using corona or tribo charging. approved plants following thermal utilisation.
Effect powder coatings are usually processed by means of
2.15 Disposal
corona charging.
Waste code in accordance with EWC: 080112 or 080201. The
Guidelines to be considered: EWC to be applied is to be specified by the waste producer.
• VDE provisions and the corresponding European
Possible disposal methods for powder coating waste are:
standards EN 16985.
1. Material utilisation, e.g. in composite materials
2. Thermal utilisation in approved systems.
Powder coatings do not contain any solvents.
2.16 Further information
The overspray can be recovered and re-used using the More detailed information on the powder coating under review
corresponding plant technology. can be found in the respective product information, safety data
3 Environmental Product Declaration - Verband der deutschen Lack- und Druckfarbenindustrie e.V. - Polyester Powder Coating
sheets and on the product manufacturers' websites.
3. LCA: Calculation rules
available were taken into consideration in the analysis.
3.1 Declared Unit Accordingly, material and energy flows with a share of less than
The declared unit is 1 kg. one per cent were also considered. Machinery, plants and
The Declaration is based on an industry-standard specific infrastructure required in the manufacturing process were not
formulation for a powder coating with polyester resin as the considered.
main component. Transport expenses for packaging and cleaning granulate are
Details on declared unit not taken into account.
Likewise special waste accounting for 0.03% and internally
Name Value Unit
recycled powder coating accounting for 0.66% are cut off.
Declared unit 1 kg
3.5 Background data
With regard to the variability of the production process, the The software system for holistic balancing GaBi Software ts
geographical representativeness, and the influence of 10.6.2.9 developed by Sphera GmbH is used for modelling the
background data and preliminary products compared to the life cycle of the declared product. The respective database is
environmental impacts caused by the actual production, the GaBi 2022, version 2022.2.
results can be considered robust.
3.6 Data quality
The data quality can be regarded as good. The primary data
The formulations are the same for all companies. Minimal
was collated in full taking consideration of all relevant flows.
variances result only from the use of different colour pigments
The background data was taken from the GaBi databases. The
(3%). All other basic materials are the same.
databases were last updated in 2022.
3.2 System boundary
Type of EPD: cradle to factory gate with Modules C1–C4 and Declared formulation: a specific composition is declared in the
Module D (A1–A3, C, D). EPD. This composition reflects the declared product and was
already determined in 2016 on the basis of a survey of member
The LCA includes the provision of raw materials (Module A1), companies and confirmed again for 2022.
transport to the production site (Module A2), and the
3.7 Period under review
manufacturing processes of the powder coating, including
Collation of the primary data refers to the period 2021 (annual
packaging (Module A3).
average).
The coating process is not the subject of the study.
3.8 Geographic Representativeness
Land or region, in which the declared product system is
Only the packaging material contains biogenic carbon. At the
manufactured, used or handled at the end of the product´s
end of life, the product is transported for disposal (Module C2)
lifespan: Europe
and subsequently disposed of (Module C4).
3.3 Estimates and assumptions
3.9 Allocation
Data sets on the upstream chains associated with
Primary data:
manufacturing basic materials are taken from the GaBi
The production process does not produce any by-products.
database. Materials for which there are no inventories available
Accordingly, no resources or environmental loads were
are approximated with data sets of similar chemicals or
allocated to ancillary products in the LCA model on which the
estimated by merging available data sets.
LCA is based.
The German residual grid mix (without renewable energies with
Background data:
guarantee of origin) used in the production phase represents a
The data sets used are listed in the background report. The
worst-case scenario for most environmental indicators, so that
allocation methods used in background data (materials and
the scope of this EPD also includes Austria and Switzerland in
energy) originating from the GaBi 2022 databases are
addition to Germany. This is due to the slightly higher potential
documented online at http://www.gabi-
environmental impacts of the German residual grid mix (without
software.com/deutsch/support/gabi/.
renewable energies with guarantee of origin) compared to the
impacts of the residual grid mixes for Austria and Switzerland. 3.10 Comparability
This methodical approach ensures the validity of the EPD for Basically, a comparison or an evaluation of EPD data is only
production in any one of these three countries. possible if all the data sets to be compared were created
according to EN 15804 and the building context, respectively
3.4 Cut-off criteria
the product-specific characteristics of performance, are taken
All operating data, i.e. all of the starting materials used in
into account. The background data comes from the GaBi
accordance with the formulation, transport thereof to the plant,
database with GaBi ts software version CUP 2022.2.
the thermal and electrical energy used, packaging materials, all
direct production waste as well as all emission measurements
4. LCA: Scenarios and additional technical information
consists of 50% biogenic carbon.
Characteristic product properties of biogenic carbon None of the products investigated contains biogenic carbon.
The calculation of the biogenic carbon content is based on the Only the packaging material contains biogenic carbon.
assumption that the absolutely dry wood and board mass
4 Environmental Product Declaration - Verband der deutschen Lack- und Druckfarbenindustrie e.V. - Polyester Powder Coating
The product is declared including 0.029 kg paper packaging, substitution, only the resulting emissions.
0.005 kg PE film and 0.036 kg wood.
Name Value Unit
End of Life (C1–C4) For thermal utilisation without energy recovery 1 kg
- Module C1: Manual deconstruction (no environmental loads)
- Module C2: An average transport distance of 50 km by truck is
Reuse, recovery and recycling potential (D), relevant
assumed.
scenario details
- Module C4: As a disposal scenario, it is assumed that powder
Module D is declared. However, since no benefits are
coating that is on the metal surface during disposal is thermally
generated for the next product systemof Module A5 or Module
disposed of when the metal is recycled (melting/incineration).
C4, it was set to 0.
No credits were considered for incineration based on energy
5 Environmental Product Declaration - Verband der deutschen Lack- und Druckfarbenindustrie e.V. - Polyester Powder Coating
5. LCA: Results
DESCRIPTION OF THE SYSTEM BOUNDARY (X = INCLUDED IN LCA; ND = MODULE OR INDICATOR NOT DECLARED; MNR =
MODULE NOT RELEVANT)
Benefits and
Construction loads beyond
Product stage Use stage End of life stage
process stage the system
boundaries
la ire ta m w a Ry lp p u s tro p s n a rT g n iru tc a fu n a M e h t m o rf tro p s n a rTe tis e h t o t e ta g y lb m e s s A e s U e c n a n e tn ia M ria p e R tn e m e c a lp e R tn e m h s ib ru fe R y g re n e la n o ita re p Oe s u re ta w la n o ita re p Oe s u n o itc u rts n o c -e Dn o itilo m e d tro p s n a rT g n is s e c o rp e ts a W la s o p s iD -e s u e R-y re v o c e R-g n ilc y c e Rla itn e to p
A1 A2 A3 A4 A5 B1 B2 B3 B4 B5 B6 B7 C1 C2 C3 C4 D
X X X MND MND MND MND MNR MNR MNR MND MND X X X X X
RESULTS OF THE LCA - ENVIRONMENTAL IMPACT according to EN 15804+A2: 1 kg polyester powder coating
Parameter Unit A1-A3 C1 C2 C3 C4 D
Global Warming Potential total (GWP-total) kg CO 2 eq 4.48E+00 0 4.31E-03 0 2.3E+00 0
Global Warming Potential fossil fuels (GWP-fossil) kg CO 2 eq 4.45E+00 0 4.12E-03 0 2.3E+00 0
Global Warming Potential biogenic (GWP-biogenic) kg CO 2 eq 2.76E-02 0 1.91E-04 0 2.01E-04 0
Global Warming Potential luluc (GWP-luluc) kg CO 2 eq 4.75E-04 0 6.71E-08 0 1.18E-05 0
Depletion potential of the stratospheric ozone layer (ODP) kg CFC11 eq 1.38E-11 0 6.26E-16 0 3.33E-13 0
Acidification potential of land and water (AP) mol H+ eq 6.97E-03 0 1.34E-05 0 6.75E-04 0
Eutrophication potential aquatic freshwater (EP-freshwater) kg P eq 1E-05 0 8.56E-10 0 8.81E-08 0
Eutrophication potential aquatic marine (EP-marine) kg N eq 1.87E-03 0 6.45E-06 0 2.09E-04 0
Eutrophication potential terrestrial (EP-terrestrial) mol N eq 2.01E-02 0 7.08E-05 0 3.22E-03 0
Formation potential of tropospheric ozone photochemical oxidants kg NMVOC
7.4E-03 0 1.24E-05 0 5.44E-04 0
(POCP) eq
Abiotic depletion potential for non fossil resources (ADPE) kg Sb eq 5.74E-07 0 2.29E-10 0 8.13E-09 0
Abiotic depletion potential for fossil resources (ADPF) MJ 9.08E+01 0 5.77E-02 0 5.76E-01 0
m3 world eq
Water use (WDP) 1.51E-01 0 4.73E-06 0 2.34E-01 0
deprived
RESULTS OF THE LCA - INDICATORS TO DESCRIBE RESOURCE USE according to EN 15804+A2: 1 kg polyester powder
coating
Parameter Unit A1-A3 C1 C2 C3 C4 D
Renewable primary energy as energy carrier (PERE) MJ 6.57E+00 0 3.35E-04 0 1.21E+00 0
Renewable primary energy resources as material utilization
MJ 1.05E+00 0 0 0 -1.05E+00 0
(PERM)
Total use of renewable primary energy resources (PERT) MJ 7.62E+00 0 3.35E-04 0 1.56E-01 0
Non renewable primary energy as energy carrier (PENRE) MJ 7.38E+01 0 5.78E-02 0 1.76E+01 0
Non renewable primary energy as material utilization (PENRM) MJ 1.7E+01 0 0 0 -1.7E+01 0
Total use of non renewable primary energy resources (PENRT) MJ 9.08E+01 0 5.78E-02 0 5.76E-01 0
Use of secondary material (SM) kg 0 0 0 0 0 0
Use of renewable secondary fuels (RSF) MJ 0 0 0 0 0 0
Use of non renewable secondary fuels (NRSF) MJ 0 0 0 0 0 0
Use of net fresh water (FW) m3 1.91E-02 0 2.85E-07 0 5.52E-03 0
RESULTS OF THE LCA – WASTE CATEGORIES AND OUTPUT FLOWS according to EN 15804+A2:
1 kg polyester powder coating
Parameter Unit A1-A3 C1 C2 C3 C4 D
Hazardous waste disposed (HWD) kg 1.85E-08 0 1.93E-13 0 6.14E-11 0
Non hazardous waste disposed (NHWD) kg 8.76E-02 0 6.95E-06 0 4.88E-02 0
Radioactive waste disposed (RWD) kg 1.26E-03 0 5.13E-08 0 1.72E-05 0
Components for re-use (CRU) kg 0 0 0 0 0 0
Materials for recycling (MFR) kg 0 0 0 0 0 0
Materials for energy recovery (MER) kg 0 0 0 0 0 0
Exported electrical energy (EEE) MJ 0 0 0 0 0 0
Exported thermal energy (EET) MJ 0 0 0 0 0 0
RESULTS OF THE LCA – additional impact categories according to EN 15804+A2-optional:
1 kg polyester powder coating
Parameter Unit A1-A3 C1 C2 C3 C4 D
Disease
Incidence of disease due to PM emissions (PM) 6.97E-08 0 7.17E-11 0 3.68E-09 0
incidence
Human exposure efficiency relative to U235 (IR) kBq U235 eq 1.59E-01 0 4.6E-06 0 1.7E-03 0
Comparative toxic unit for ecosystems (ETP-fw) CTUe 5.73E+01 0 4.59E-02 0 2.19E-01 0
6 Environmental Product Declaration - Verband der deutschen Lack- und Druckfarbenindustrie e.V. - Polyester Powder Coating
Comparative toxic unit for humans (carcinogenic) (HTP-c) CTUh 1.79E-09 0 8.61E-13 0 2.36E-11 0
Comparative toxic unit for humans (noncarcinogenic) (HTP-nc) CTUh 1.63E-07 0 4.33E-11 0 1.5E-09 0
Soil quality index (SQP) SQP 1.49E+01 0 2.51E-04 0 1.62E-01 0
Limitation note 1 – applies to the indicator 'Potential impact from human exposure to U235'. This impact category mainly addresses the
potential effect of low-dose ionising radiation on human health in the nuclear fuel cycle. It does not consider effects due to possible
nuclear accidents and occupational exposure, nor does it consider effects due to the disposal of radioactive waste in underground
facilities. Potential ionising radiation from soil, radon and some building materials is also not measured by this indicator.
Limitation note 2 – applies to the indicators: 'Potential for depletion of abiotic resources – non-fossil resources', 'Potential for depletion
of abiotic resources – fossil fuels', 'Water depletion potential (user)', 'Potential toxicity comparison unit for ecosystems', 'Potential
toxicity comparison unit for humans – carcinogenic effect', 'Potential toxicity comparison unit for humans – non-carcinogenic effect',
'Potential soil quality index'. The results of this environmental impact indicator need to be used with caution as the uncertainties in
these results are high or as there is limited experience with the indicator.
6. LCA: Interpretation
The loads in the production phase are dominated by the agent is the main cause of Acidification Potential of Soil and
upstream chain associated with the raw material supply. The Water (AP) and Abiotic Depletion Potential of non-fossil
use of ancillaries and energy has a minor influence. resources (ADP elements).
Transport has a negligible influence. The environmental loads
within raw material supply (A1) are primarily dominated by the The End-of-Life scenario (C4), which considers the waste
binding agent and titanium dioxide in the various environmental incineration plant process, also shows relevant impacts.
impact categories. As in all other impact categories, the binding
7. Requisite evidence
The powder coating outlined in this EPD is used in interior coatings as they involve preliminary products which are only
applications, among others. Evidence in terms of consumer used following application on a substrate in the building.
protection inside buildings is not of relevance for powder
8. References
Standards:
ISO 6270-1
EN 12206-1 DIN EN ISO 6270-1:2018-04, Paints and varnishes –
DIN EN 12206-1:2021-07, Paints and varnishes – Coating of Determination of resistance to humidity – Part 1: Condensation
aluminium and aluminium alloys for architectural purposes – (single-sided exposure)
Part 1: Coatings prepared from thermosetting coating powder
ISO 8130-2
EN 13501-1 DIN EN ISO 8130-2:2021-10, Coating powders – Part 2:
DIN EN 13501-1:2019-05, Fire classification of construction Determination of density by gas comparison pycnometer
products and building elements – Part 1: Classification using (referee method)
data from reaction to fire tests
ISO 9227
EN 15804 DIN EN ISO 9227:2017-07, Corrosion tests in artificial
DIN EN 15804:2022-03, Sustainability of construction works – atmospheres – Salt spray tests
Environmental product declarations – Core rules for the product
category of construction products ISO 14001
DIN EN ISO 14001:2015-11, Environmental management
EN 16985 systems – Requirements with guidance for use
DIN EN 16985:2019-04, Spray booths for organic coating
material – Safety requirements ISO 14004
DIN EN ISO 14004:2016-08, Environmental management
ISO 1519 systems – General guidelines on implementation
DIN EN ISO 1519:2011-04, Paints and varnishes – Bend test
(cylindrical mandrel) ISO 16474-3
DIN EN ISO 16474-3:2021-04, Paints and varnishes – Methods
ISO 1520 of exposure to laboratory light sources – Part 3: Fluorescent UV
DIN EN ISO 1520:2007-11, Paints and varnishes – Cupping lamps
test
ISO 2813 Other sources:
DIN EN ISO 2813:2015-02, Paints and varnishes –
Determination of gloss value at 20 degrees, 60 degrees and 85 Biocidal Products Regulation
degrees Regulation (EU) No 528/2012 of the European Parliament and
of the Council of 22 May 2012 concerning the making available
ISO 3251 on the market and use of biocidal products.
DIN EN ISO 3251:2019-09, Paints, varnishes and plastics –
Determination of non-volatile matter content CLP Regulation
7 Environmental Product Declaration - Verband der deutschen Lack- und Druckfarbenindustrie e.V. - Polyester Powder Coating
Regulation (EC) No 1272/2008 of the European Parliament and PCR, Part A
of the Council of 16 December 2008 on classification, labelling Product Category Rules for building-related products and
and packaging of substances and mixtures, amending and services. Part A: Calculation rules for the Life Cycle
repealing Directives 67/548/EEC and 1999/45/EC, and Assessment and requirements on the Project Report, Berlin:
amending Regulation (EC) No. Institut Bauen und Umwelt e.V. (pub.), version 1.3, 08/2022
1907/2006 (www.ibu-epd.com)
ECHA Candidate List PCR: Coatings with organic binding agents
Candidate List of Substances of Very High Concern for Product Category Rules for building-related products and
Authorisation (ECHA Candidate List), dated 10.06.2022, services. Part B: Requirements on the EPD for coatings with
published in accordance with Article 59 (10) of the REACH organic binding agents, Institut Bauen und Umwelt e.V.,
Regulation. Helsinki: European Chemicals Agency. www.ibu-epd.com, version 1, 04/2023.
EC Eco-Audit Regulation
Regulation (EC) No. 1221/2009 of the European Parliament The specialist group for powder coatings of the Verband
and of the Council of 25 November 2009 on the voluntary der deutschen Lack- und Druckfarbenindustrie e.V.
participation by organisations in a Community eco-management (German Paint and Printing Ink Industry Association
and audit scheme (EMAS), repealing Regulation (EC) No. (VdL)), which is made up of the following companies, was
761/2001 and Commission Decisions 2001/681/EC and involved in the preparation of the EPD:
2006/193/EC
Akzo Nobel Powder Coatings GmbH, production sites:
EMAS Regulation Arnsberg, Reutlingen
Regulation (EC) No. 761/2001 of the European Parliament and
of the Council of 19 March 2001 allowing voluntary participation Axalta Coating Systems Germany GmbH, production site:
by organisations in a Community eco-management and audit Essenbach-Altheim
scheme (EMAS)
CWS Powder Coatings GmbH, production site: Düren
EWC
European Waste Code (EWC), No. 080112 – paint and varnish Emil Frei GmbH & Co. KG, production site: Bräunlingen-
waste with the exception of those covered by 08 01 11, Döggingen
European Waste Code (EWC), No. 080201 – Coating powder
waste, Regulation on the European Waste Catalogue (EWC) Ganzlin Beschichtungspulver GmbH, production site:
dated 10 December 2001 Ganzlin
GaBi documentation Helios Coatings Deutschland GmbH, production site:
GaBi life cycle inventory data documentation; Buchholz
https://www.gabisoftware.com/support/gabi/gabidatabase2020lcidocumentation/
INVER GmbH, production sites: none in DACH
GaBi
Sphera Solutions GmbH, GaBi Software System and Database Karl Bubenhofer AG Farbenfabrik, production site: Arnegg
for Life Cycle Engineering, CUP version: 2022.2, University of (CH)
Stuttgart, Leinfelden Echterdingen
Karl Wörwag Lack- und Farbenfabrik GmbH & Co. KG,
IBU 2021 production sites Renningen
General EPD range instructions of Institut Bauen und Umwelt
e.V. (IBU), version 2.0, Berlin: Institut Bauen und Umwelt e.V., RIPOL GmbH, production sites: none in DACH
2021; www.ibu-epd.com
TIGER Coatings GmbH & Co. KG, Pproduction site: Wels (A)
8 Environmental Product Declaration - Verband der deutschen Lack- und Druckfarbenindustrie e.V. - Polyester Powder Coating
Publisher
Institut Bauen und Umwelt e.V. +49 (0)30 3087748- 0
Hegelplatz 1 info@ibu-epd.com
10117 Berlin www.ibu-epd.com
Germany
Programme holder
Institut Bauen und Umwelt e.V. +49 (0)30 3087748- 0
Hegelplatz 1 info@ibu-epd.com
10117 Berlin www.ibu-epd.com
Germany
Author of the Life Cycle Assessment
Sphera Solutions GmbH +49 711 341817-0
Hauptstraße 111- 113 info@sphera.com
70771 Leinfelden-Echterdingen www.sphera.com
Germany
Owner of the Declaration
VdL - Verband der deutschen Lack- und +49 69 2556-1411
Druckfarbenindustrie e.V. vdl@vci.de
Mainzer Landstraße 55 www.wirsindfarbe.de
60329 Frankfurt a. M.
Germany
9 Environmental Product Declaration - Verband der deutschen Lack- und Druckfarbenindustrie e.V. - Polyester Powder Coating
