ENVIRONMENTAL PRODUCT DECLARATION
as per ISO 14025 and EN 15804+A2
Owner of the Declaration Sika Services AG
Publisher Institut Bauen und Umwelt e.V. (IBU)
Programme holder Institut Bauen und Umwelt e.V. (IBU)
Declaration number EPD-SIK-20240200-IBA2-EN
Issue date 29/07/2024
Valid to 28/07/2029
SikaMembran-820 / 800
Sika Services AG
www.ibu-epd.com | https://epd-online.com
General Information
Sika Services AG SikaMembran-820 / 800
Programme holder Owner of the declaration
IBU – Institut Bauen und Umwelt e.V. Sika Services AG
Hegelplatz 1 Tüffenwies 16-22
10117 Berlin 8064 Zurich
Germany Switzerland
Declaration number Declared product / declared unit
EPD-SIK-20240200-IBA2-EN 1 m2 SikaMembran®-820/800 waterproofing and vapour control
membrane.
This declaration is based on the product category rules: Scope:
Plastic and elastomer roofing and sealing sheet systems, This document applies to SikaMembran®-820 and SikaMembran®-800
01/08/2021 waterproofing and vapour control membrane in thickness of 0.3 mm,
(PCR checked and approved by the SVR) manufactured by Sika Manufacturing AG in DE-53840 Troisdorf, Germany.
There are two membranes from Sika considered in this study
(SikaMembran 800 and SikaMembran 820). SikaMembran 820 is non-
Issue date perforated membrane, which is produced with the same recipe and
production processes as SikaMembran 800 (perforated membrane; except
29/07/2024
perforation process). The EPD declares a worst case scenario which is
calculated for one of the variations - SikaMembran 800 (perforated
membrane) that can also cover SikaMembran 820 (non-perforated
Valid to
membrane).
28/07/2029
The owner of the declaration shall be liable for the underlying information
and evidence; the IBU shall not be liable with respect to manufacturer
information, life cycle assessment data and evidences.
The EPD was created according to the specifications of EN 15804+A2. In
the following, the standard will be simplified as EN 15804.
Verification
The standard EN 15804 serves as the core PCR
Independent verification of the declaration and data according to ISO
Dipl.-Ing. Hans Peters
14025:2011
(Chairman of Institut Bauen und Umwelt e.V.)
internally X externally
Florian Pronold Matthias Schulz,
(Managing Director Institut Bauen und Umwelt e.V.) (Independent verifier)
1 Environmental Product Declaration - Sika Services AG - SikaMembran-820 / 800
Product
Additional technical data are not relevant for this product.
Product description/Product definition
SikaMembran®-820/800 is a polymeric waterproofing and Performance values of the product in accordance with the
vapour control membrane, an elastic EPDM Hybrid and is Declaration of Performance with regard to its essential
treated with stabilizers against UV radiation. characteristics as defined by DIN EN 13984:2013, Flexible
sheets for waterproofing – Plastic and rubber vapour control
SikaMembran®-820/800 is available in the thickness of 0.3 mm layers.
and in single rolls of different widths.
Base materials/Ancillary materials
SikaMembran 820 is non- perforated membrane, which is The raw materials and additives of SikaMembran®-820/800
produced with the same recipe and production processes as waterproofing and vapour control membrane can be given as
SikaMembran 800 (perforated membrane; except perforation follows:
process). The EPD declares a worst case scenario which is • Polymer including elastomer 75-85 %
calculated for one of the variations - SikaMembran 800 • Mineral Flame retardant 10-20 %
(perforated membrane) that can also cover SikaMembran 820 • Stabilizer 0.1-0.5 %
(non-perforated membrane). • Pigments: 0–5 %
This product contains substances listed in the candidate
For the placing on the market of the product in the European list (date: 20.04.2023) exceeding 0.1 percentage by
Union/European Free Trade Association (EU/EFTA) (with the mass: No
exception of Switzerland) Regulation (EU) No. 305/2011 (CPR) This product contains other CMR substances in
applies. The product needs a declaration of performance taking categories 1A or 1B which are not on the candidate list,
into consideration EN 13984:2013, Flexible sheets for exceeding 0.1 percentage by mass: No
waterproofing – Plastic and rubber vapour control layers - and Biocide products were added to this construction
the CE-marking. product or it has been treated with biocide products (this
then concerns a treated product as defined by the (EU)
Ordinance on Biocide Products No. 528/2012): No
Application
SikaMembran®-820/800 systems provide a secure and durable
vapour barrier and waterproof seal at junctions between Reference service life
building elements mainly in curtain wall facades but also in The service life depends on climatic conditions and the
ventilated facades and window installations. The membrane is installation in the building. Based on the study Durability of
attached to the building elements with a pasty adhesive on all Sarnafil® T Polymeric Waterproofing Membranes from 2014, it
four sides. is reasonable to expect a service life of up to 50 years for the
SikaMembran®-820/800, assuming correct application and
Technical Data
maintenance.
Constructional data This finding reflects the product's high resistance to weathering
SikaMembran®-820 and ageing when used properly.
Name Value Unit
Tensile strength as per EN 12311-2 10 N
Elongation as per EN 12311-2 > 600 %
Tear propagation resistance as per EN 12310-1 85 N
Artificial ageing as per EN 1297 passed -
Dimensional stability as per EN 1107-2 ≤ 1.6 %
Chemical Resistance as per EN 1847 passed
LCA: Calculation rules
Declared Unit System boundary
Name Value Unit Declaration type with respect to life cycle stages covered
Grammage 0.34 kg/m2 according to clause 5.2 EN 15804+A2 is cradle to gate with
modules C1–C4 and module D (A1–A3, A4, A5, C and D).
Declared unit 1 m2
Layer thickness 0.0003 m
The EPD declares a worst case scenario which is calculated for
Module A1 to A3:
one of the variations - SikaMembran 800 (perforated
The product stage includes provision of all materials, products
membrane) that can also cover SikaMembran 820 (non-
and energy, as well as waste processing up to the end-of waste
perforated membrane). The model was calculated on the basis
state or disposal of final residues during the product stage.
of production data for the thickness 0.3 mm provided by Sika
These modules consider the manufacturing of system
Technology AG from the year 2022.
components/raw materials, the transport to the production site
and the production processes/manufacturing/assembly of the
Other declared units are allowed if the conversion is shown
product under study. The impact of packaging materials is
transparently.
included.
2 Environmental Product Declaration - Sika Services AG - SikaMembran-820 / 800
Module D:
Module A4: For the thermal and electrical energy generated in Module A5
This module considers 100 km truck transport to site (diesel and C3 due to thermal treatment of packaging and product
driven, EURO 6, 40 tons total load, 61% utilization). The waste, avoided burdens have been calculated by the inversion
transport distance can be modified project specific if required by of electricity grid mix and thermal energy from natural gas,
linear scaling. using German datasets.
As a conservative approach, credits are only given to the
Module A5: incineration of the plastic parts in order not to overestimate the
Installation of membranes is considered manually, with benefits from the product incineration.
negligible amount of adhesive. Treatment and disposal of
packaging material. Credits for potential avoided burdens due Geographic Representativeness
to energy substitution of electricity and thermal energy Land or region, in which the declared product system is
generation are declared in module D and affects only the rate of manufactured, used or handled at the end of the product´s
primary material (no secondary materials). lifespan: Germany
Module C1 to C4:
Comparability
• Manual dismantling → no loads (C1).
Basically, a comparison or an evaluation of EPD data is only
• 50 km transport by 40 to truck, EURO 6, 61% average
possible if all the data sets to be compared were created
utilization (C2).
according to EN 15804 and the building context, respectively
• Thermal treatment of materials (C3) with heating
the product-specific characteristics of performance, are taken
value >2 MJ/kg in MWI plants, assuming an R1 value
into account. Background database: LCAFE Software
of >0.6
Database 2023.2
• The membrane is not subjected to landfill (C4), hence
landfill scenario (C4) is not relevant.
LCA: Scenarios and additional technical information
Installation into the building (A5)
Characteristic product properties of biogenic carbon
Name Value Unit
Name Value Unit
Output substances following waste treatment on
kg 0.02795 kg
Biogenic carbon content in product - site - Wooden Pallets
C
Biogenic carbon content in accompanying 0.01118 kg End of life (C1-C4)
packaging C
Name Value Unit
Collected separately waste type 0.34 kg
Note: 1 kg of biogenic carbon is equivalent to 44/12 kg of CO2.
Energy recovery 0.34 kg
Transport to the building site (A4)
Reuse, recovery and/or recycling potentials (D), relevant
Name Value Unit scenario information
Litres of fuel 0.0018 l/100km Module D includes the potential benefits in form of energy
Transport distance 100 km recovery of the incineration process in A5 (incineration of
Capacity utilisation (including empty runs) 61 % packaging wastes) and C3 (combustion of the product).
3 Environmental Product Declaration - Sika Services AG - SikaMembran-820 / 800
LCA: Results
DESCRIPTION OF THE SYSTEM BOUNDARY (X = INCLUDED IN LCA; MND = MODULE OR INDICATOR NOT DECLARED; MNR
= MODULE NOT RELEVANT)
Benefits and
Construction loads beyond
Product stage Use stage End of life stage
process stage the system
boundaries
la ire ta m w a Ry lp p u s tro p s n a rT g n iru tc a fu n a M e h t m o rf tro p s n a rTe tis e h t o t e ta g y lb m e s s A e s U e c n a n e tn ia M ria p e R tn e m e c a lp e R tn e m h s ib ru fe R y g re n e la n o ita re p Oe s u re ta w la n o ita re p Oe s u n o itc u rts n o c -e Dn o itilo m e d tro p s n a rT g n is s e c o rp e ts a W la s o p s iD -e s u e R-y re v o c e R-g n ilc y c e Rla itn e to p
A1 A2 A3 A4 A5 B1 B2 B3 B4 B5 B6 B7 C1 C2 C3 C4 D
X X X X X MND MND MNR MNR MNR MND MND X X X X X
RESULTS OF THE LCA - ENVIRONMENTAL IMPACT according to EN 15804+A2: 1 m² SikaMembran®-820/800
Parameter Unit A1-A3 A4 A5 C1 C2 C3 C4 D
GWP-total kg CO 2 eq 9.08E-01 2.99E-03 4.28E-02 0 1.38E-03 7.83E-01 0 -2.44E-01
GWP-fossil kg CO 2 eq 9.48E-01 2.96E-03 8.36E-04 0 1.37E-03 7.81E-01 0 -2.43E-01
GWP-biogenic kg CO 2 eq -4.07E-02 8.43E-06 4.2E-02 0 3.89E-06 1.94E-03 0 -1.77E-03
GWP-luluc kg CO 2 eq 4.41E-04 1.79E-05 1.95E-07 0 8.29E-06 4.48E-06 0 -2.24E-05
ODP kg CFC11 eq 5.52E-08 7.4E-16 7.67E-15 0 3.42E-16 1.23E-13 0 -3E-12
AP mol H+ eq 1.15E-03 2.53E-06 8.66E-06 0 1.17E-06 2.29E-04 0 -2.47E-04
EP-freshwater kg P eq 1.6E-06 7.07E-09 2.01E-09 0 3.27E-09 3.43E-08 0 -6.64E-07
EP-marine kg N eq 3.32E-04 7.25E-07 2.19E-06 0 3.35E-07 7.09E-05 0 -9.13E-05
EP-terrestrial mol N eq 3.65E-03 9.26E-06 3.72E-05 0 4.28E-06 1.1E-03 0 -9.7E-04
kg NMVOC
POCP 1.43E-03 2.14E-06 5.8E-06 0 9.87E-07 1.85E-04 0 -2.34E-04
eq
ADPE kg Sb eq 3.45E-06 2.17E-10 5.76E-11 0 1E-10 9.25E-10 0 -2.13E-08
ADPF MJ 2.67E+01 4.08E-02 1.13E-02 0 1.88E-02 2.04E-01 0 -3.81E+00
m3 world eq
WDP 3E-02 1.57E-05 4.67E-03 0 7.28E-06 7.97E-02 0 -3.23E-03
deprived
GWP = Global warming potential; ODP = Depletion potential of the stratospheric ozone layer; AP = Acidification potential of land and water; EP =
Eutrophication potential; POCP = Formation potential of tropospheric ozone photochemical oxidants; ADPE = Abiotic depletion potential for non-fossil
resources; ADPF = Abiotic depletion potential for fossil resources; WDP = Water (user) deprivation potential)
RESULTS OF THE LCA - INDICATORS TO DESCRIBE RESOURCE USE according to EN 15804+A2: 1 m² SikaMembran®-
820/800
Parameter Unit A1-A3 A4 A5 C1 C2 C3 C4 D
PERE MJ 1.37E+00 2.73E-03 4.06E-01 0 1.26E-03 8.37E-02 0 -1.46E+00
PERM MJ 4.26E-01 0 -4.02E-01 0 0 -2.33E-02 0 0
PERT MJ 1.8E+00 2.73E-03 3.75E-03 0 1.26E-03 6.04E-02 0 -1.46E+00
PENRE MJ 1.23E+01 4.09E-02 1.13E-02 0 1.89E-02 1.46E+01 0 -3.81E+00
PENRM MJ 1.44E+01 0 0 0 0 -1.44E+01 0 0
PENRT MJ 2.67E+01 4.09E-02 1.13E-02 0 1.89E-02 2.05E-01 0 -3.81E+00
SM kg 0 0 0 0 0 0 0 0
RSF MJ 0 0 0 0 0 0 0 0
NRSF MJ 0 0 0 0 0 0 0 0
FW m3 3.42E-03 2.43E-06 1.1E-04 0 1.12E-06 1.88E-03 0 -5.19E-04
PERE = Use of renewable primary energy excluding renewable primary energy resources used as raw materials; PERM = Use of renewable primary
energy resources used as raw materials; PERT = Total use of renewable primary energy resources; PENRE = Use of non-renewable primary energy
excluding non-renewable primary energy resources used as raw materials; PENRM = Use of non-renewable primary energy resources used as raw
materials; PENRT = Total use of non-renewable primary energy resources; SM = Use of secondary material; RSF = Use of renewable secondary fuels;
NRSF = Use of non-renewable secondary fuels; FW = Use of net fresh water
RESULTS OF THE LCA – WASTE CATEGORIES AND OUTPUT FLOWS according to EN 15804+A2:
1 m² SikaMembran®-820/800
Parameter Unit A1-A3 A4 A5 C1 C2 C3 C4 D
HWD kg 2.32E-09 6.89E-14 4.71E-14 0 3.18E-14 3.25E-12 0 -2.3E-10
NHWD kg 1.18E-02 6.12E-06 6.18E-04 0 2.83E-06 1.67E-02 0 -2.05E-03
RWD kg 3E-04 5.38E-08 3.87E-07 0 2.48E-08 6.22E-06 0 -1.51E-04
CRU kg 0 0 0 0 0 0 0 0
MFR kg 0 0 0 0 0 0 0 0
MER kg 0 0 0 0 0 0 0 0
EEE MJ 0 0 5.02E-02 0 0 8.51E-01 0 0
EET MJ 0 0 1.18E-01 0 0 1.95E+00 0 0
4 Environmental Product Declaration - Sika Services AG - SikaMembran-820 / 800
HWD = Hazardous waste disposed; NHWD = Non-hazardous waste disposed; RWD = Radioactive waste disposed; CRU = Components for re-use;
MFR = Materials for recycling; MER = Materials for energy recovery; EEE = Exported electrical energy; EET = Exported thermal energy
RESULTS OF THE LCA – additional impact categories according to EN 15804+A2-optional:
1 m² SikaMembran®-820/800
Parameter Unit A1-A3 A4 A5 C1 C2 C3 C4 D
Disease
PM 1.38E-08 1.88E-11 5.77E-11 0 8.67E-12 1.25E-09 0 -1.79E-09
incidence
IR kBq U235 eq 2.72E-02 5.76E-06 4.09E-05 0 2.66E-06 6.57E-04 0 -1.6E-02
ETP-fw CTUe 1.12E+01 2.98E-02 4.37E-03 0 1.38E-02 7.43E-02 0 -5.98E-01
HTP-c CTUh 2.93E-10 5.94E-13 4.12E-13 0 2.74E-13 8.27E-12 0 -4.64E-11
HTP-nc CTUh 1.19E-08 2.49E-11 1.83E-11 0 1.15E-11 3.77E-10 0 -1.24E-09
SQP SQP 7.71E+00 1.45E-02 4E-03 0 6.71E-03 6.15E-02 0 -1.01E+00
PM = Potential incidence of disease due to PM emissions; IR = Potential Human exposure efficiency relative to U235; ETP-fw = Potential comparative
Toxic Unit for ecosystems; HTP-c = Potential comparative Toxic Unit for humans (cancerogenic); HTP-nc = Potential comparative Toxic Unit for humans
(not cancerogenic); SQP = Potential soil quality index
Disclaimer 1 – for the indicator “Potential Human exposure efficiency relative to U235”. This impact category deals mainly with the
eventual impact of low-dose ionizing radiation on human health of the nuclear fuel cycle. It does not consider effects due to possible
nuclear accidents, occupational exposure or radioactive waste disposal in underground facilities. Potential ionizing radiation from the
soil, radon and from some construction materials is also not measured by this indicator.
Disclaimer 2 – for the indicators “abiotic depletion potential for non-fossil resources”, “abiotic depletion potential for fossil resources”,
“water (user) deprivation potential, deprivation-weighted water consumption”, “potential comparative toxic unit for ecosystems”,
“potential comparative toxic unit for humans – cancerogenic”, “Potential comparative toxic unit for humans - not cancerogenic”,
“potential soil quality index”. The results of this environmental impact indicator shall be used with care as the uncertainties on these
results are high as there is limited experience with the indicator.
References
Regulation (EU) No. 305/2011 (CPR) EN 15804:2012+A2:2019+AC:2021, Sustainability of
of the European Parliament and of the Council of 9 March 2011 construction works — Environmental Product Declarations —
laying down harmonised conditions for the marketing of Core rules for the product category of construction products.
construction products and repealing Council Directive
89/106/EEC Text with EEA relevance. ISO 14025
EN ISO 14025:2011, Environmental labels and declarations —
DIN EN 13948:2013 Type III environmental declarations — Principles and
Flexible sheets for waterproofing – Plastic and rubber vapour procedures.
control layers
IBU 2021
EN 12311-2 Institut Bauen und Umwelt e.V.: General Instructions for the
Flexible Sheets For Waterproofing - Determination Of Tensile EPD programme of Institut Bauen und Umwelt e.V., Version
and Elongation Properties - Part 2: Plastic And Rubber Sheets 2.0, Berlin: Institut Bauen und Umwelt e.V., 2021
For Roof Waterproofing www.ibu-epd.com
EN 12310-1 IBU PART A
Flexible Sheets For Waterproofing - Determination Of PCR - Part A: Calculation Rules for the Life Cycle Assessment
Resistance To Tearing. and Requirements on the Project Report according to EN
15804+A2:2019, version 1.3, Institut Bauen und Umwelt e.V.,
EN 1297 www.bau-umwelt.com, 31/08/2022
Flexible sheets for waterproofing - Bitumen, plastic and rubber
sheets for roof waterproofing - Method of artificial ageing by IBU Part B
long term exposure to the combination of UV radiation, PCR – Part B: Requirements of the EPD for Plastic and
elevated temperature and water. elastomer roofing and sealing sheet systems, version 8, Institut
Bauen und Umwelt e.V., www.bau-umwelt.com, 30/04/2024
EN 1107-2
Flexible sheets for waterproofing - Determination of
dimensional stability - Part 2: Plastic and rubber sheets for roof LCAFE software
waterproofing. Sphera Solutions GmbH, GaBi Software System and Database
for Life Cycle Engineering CUP Version: 2023.1University of
EN 1847 Stuttgart Leinfelden Echterdingen
Flexible sheets for waterproofing - Plastics and rubber sheets
for roof waterproofing - Methods for exposure to liquid LCAFE documentation
chemicals, including water. LCAFE life cycle inventory data
documentation(https://sphera.com/product-sustainability-gabi-
EN 15804 data-search/)
EN 15804:2012+A1 2013, Sustainability of construction works
— Environmental Product Declarations — Core rules for the REACH
product category of construction products. Directive (EC) No. 1907/2006 of the European Parliament and
Council of 18 December 2006 on the Registration, Evaluation,
EN 15804 Authorisation of Chemicals (REACH) for establishing a
5 Environmental Product Declaration - Sika Services AG - SikaMembran-820 / 800
European Chemicals Agency
6 Environmental Product Declaration - Sika Services AG - SikaMembran-820 / 800
Publisher
Institut Bauen und Umwelt e.V. +49 (0)30 3087748- 0
Hegelplatz 1 info@ibu-epd.com
10117 Berlin www.ibu-epd.com
Germany
Programme holder
Institut Bauen und Umwelt e.V. +49 (0)30 3087748- 0
Hegelplatz 1 info@ibu-epd.com
10117 Berlin www.ibu-epd.com
Germany
Author of the Life Cycle Assessment
Sphera Solutions GmbH +49 (0)711 341817-0
Hauptstraße 111- 113 info@sphera.com
70771 Leinfelden-Echterdingen www.sphera.com
Germany
Owner of the Declaration
Sika Services AG +41(0)58 436 40 40
Tüffenwies 16-22 product.sustainability@ch.sika.com
8064 Zurich https://www.sika.com/
Switzerland
7 Environmental Product Declaration - Sika Services AG - SikaMembran-820 / 800
