ENVIRONMENTAL PRODUCT DECLARATION
as per ISO 14025 and EN 15804+A2
Owner of the Declaration dormakaba International Holding GmbH
Publisher Institut Bauen und Umwelt e.V. (IBU)
Programme holder Institut Bauen und Umwelt e.V. (IBU)
Declaration number EPD-DOR-20220039-CBA1-EN
Issue date 04.05.2022
Valid to 03.05.2027
Precision 2000 Series
dormakaba
www.ibu-epd.com | https://epd-online.com
General Information
dormakaba Precision 2000 Series
Programme holder Owner of the declaration
IBU – Institut Bauen und Umwelt e.V. dormakaba International Holding GmbH
Hegelplatz 1 DORMA Platz 1
10117 Berlin 58256 Ennepetal
Germany Germany
Declaration number Declared product / declared unit
EPD-DOR-20220039-CBA1-EN 1 exit device (1 piece) of the Precision 2000 Series.
This declaration is based on the product category rules: Scope:
Building Hardware products, 01.08.2021 This Environmental Product Declaration refers to a specific exit device
(PCR checked and approved by the SVR) manufactured by dormakaba. The production site is located in Indianapolis
(USA).
Issue date The data represents the year 2020.
The owner of the declaration shall be liable for the underlying information
04.05.2022
and evidence; the IBU shall not be liable with respect to manufacturer
information, life cycle assessment data and evidences.
Valid to
The EPD was created according to the specifications of EN 15804+A2. In
03.05.2027 the following, the standard will be simplified as EN 15804.
Verification
The standard EN 15804 serves as the core PCR
Independent verification of the declaration and data according to ISO
14025:2011
internally X externally
Dipl.-Ing. Hans Peters
(Chairman of Institut Bauen und Umwelt e.V.)
Florian Pronold Dr.-Ing. Wolfram Trinius,
(Managing Director Institut Bauen und Umwelt e.V.) (Independent verifier)
1 Environmental Product Declaration - dormakaba - Precision 2000 Series
Product
Performance data of the product with respect to its
Product description/Product definition characteristics in accordance with the relevant technical
No other exit device offers the level of functionality and provision which can be applied are mentioned above.
dependability as this Grade 1, heavy-duty exit device. Built with
fewer components and in various door configurations, the Base materials/Ancillary materials
Precision 2000 provides smoother operation with minimal need Name Value Unit
for maintenance. The Precision 2000's durable construction
Stainless steel 43 %
allows it to withstand high traffic and high use on a regular
Steel 30 %
basis, making it particularly attractive for healthcare and
Brass 14 %
education buildings. These combined benefits give it a longer
life span and a lower overall cost of ownership. For the use and Paper 6 %
application of the product the respective national provisions at Electronics 5 %
the place of use apply. The standards which can be applied are Zinc 2 %
the following:
Other <1 %
• ANSI/BHMA A156.3 Grade 1
The product/s include/s partial articles which contain
• ANSI A117.1 Accessibility Code (ADA) compliant
substances listed in the Candidate List of REACH Regulation
• UL/cUL listed
1907/2006/EC (date: 17.01.2022) exceeding 0.1 percentage by
• Florida Building Code compliant for hurricanes
mass: yes
• Miami-Dade County compliant for hurricanes
• California State Fire Marshal (California Title 24) • Lead (Pb): 7439-92-1 (CAS-No.) is included in some of
compliant the alloys used. The concentration of lead in each
• California State Fire Marshal compliant for fire door individual alloy does not exceed 4.0% (by mass).
• BAA and TAA compliant The Candidate List can be found on the ECHA website
• Illinois Accessibility Standard compliant address: https://echa.europa.eu/de/home.
Application Reference service life
The Precision 2000 Series can be used for following building The reference service life of the Precision 2000 Series exit
types: device depends on the traffic pattern and degree of usage of
the door. These exits are rated to ANSI Grade 1, meaning they
• Learning and higher education
are designed to withstand a minimum of 500,000 cycles.
• Healthcare
However, these exits have been independently tested to
• Government
surpass 10,000,000 cycles.
• Retail and commercial
• Multifamily
• Hospitality
Technical Data
The exit device has following technical properties:
2 Environmental Product Declaration - dormakaba - Precision 2000 Series
LCA: Calculation rules
construction process stage.
Declared Unit
The declared unit is 1 piece of the product: Precision 2000 End-of-life stage– Modules C1-C4 and D
Series. The end-of-life stage includes:
Declared unit — C1, de-construction, demolition:
— C2, transport to waste processing;
Name Value Unit
— C3, waste processing for reuse, recovery and/or recycling;
Declared unit 1 piece/product
— C4, disposal;
Mass of declared Product 12.04 kg including provision and all transport, provision of all materials,
products and related energy and water use.
System boundary
The type of EPD is: cradle to gate with options, modules C1–
C4, and module D (A1–A3 + C + D and additional modules: A4 Module D (Benefits and loads beyond the system boundary)
+ A5) includes:
— D, recycling potentials, expressed as net impacts and
Production - Module A1-A3 benefits.
The product stage includes:
Geographic Representativeness
— A1, raw material extraction, processing and mechanical
Land or region, in which the declared product system is
treatments, processing of secondary material input (e.g.
manufactured, used or handled at the end of the product´s
recycling processes), — A2, transport to the manufacturer,
lifespan: United States
— A3, manufacturing and assembly including provision of all
materials, products and energy, as well as waste processing up
to the end-of waste state.
Comparability
Basically, a comparison or an evaluation of EPD data is only
Construction stage - Modules A4-A5
possible if all the data sets to be compared were created
The construction process stage includes:
according to EN 15804 and the building context, respectively
— A4, transport to the building site;
the product-specific characteristics of performance, are taken
— A5, installation into the building; including provision of all
into account.
materials, products and energy, as well as waste processing up
to the end-of waste state or disposal of final residues during the
LCA: Scenarios and additional technical information
Operational energy use (B6)
Characteristic product properties of biogenic carbon
Name Value Unit
Information on describing the biogenic Carbon Content at
Electricity consumption for 1 year 62,41 kWh
factory gate
Power consumpiton "on mode" 570 W
Name ValueUnit
Hours per day in use "on mode" 0,3 h
kg
Biogenic carbon content in product 0.01 C Power consumption "standby mode" 0 W
Biogenic carbon content in accompanying kg Hours per day in use "standby mode" 23,7 h
0.09
packaging C
End of life (C1-C4)
Note: 1 kg of biogenic carbon is equivalent to 44/12 kg of CO 2. C1: The product dismantling from the building is done manually
without environmental burden.
C2: Transport to waste treatment at end of life is 50km.
Additional technical information for the declared modules.
Name Value Unit
Transport to the building site (A4) Collected separately waste type 11.3 kg
Name Value Unit Recycling 10.7 kg
Litres of fuel per 1 kg (truck) 0.00276l/100km Energy recovery 0.012 kg
Transport distance (truck) 4300 km Final deposition 0,609 kg
Capacity utilisation (including empty runs)
55 % Reuse, recovery and/or recycling potentials (D), relevant
average
scenario information
Transport distance (ship) 27000 km
Name Value Unit
Installation into the building (A5)
Collection rate is 100%.
Name ValueUnit
Output substances following waste treatment on
0.69 kg
site (packaging)
3 Environmental Product Declaration - dormakaba - Precision 2000 Series
LCA: Results
Disclaimer:
EP-freshwater: This indicator has been calculated as 'kg P eq' as required in the characterization model (EUTREND model, Struijs et
al., 2009b, as implemented in ReCiPe; http://eplca.jrc.ec.europa.eu/LCDN/developerEF.xhtml)
DESCRIPTION OF THE SYSTEM BOUNDARY (X = INCLUDED IN LCA; MND = MODULE OR INDICATOR NOT DECLARED; MNR
= MODULE NOT RELEVANT)
Benefits and
Construction loads beyond
Product stage Use stage End of life stage
process stage the system
boundaries
la ire ta m w a Ry lp p u s tro p s n a rT g n iru tc a fu n a M e h t m o rf tro p s n a rTe tis e h t o t e ta g y lb m e s s A e s U e c n a n e tn ia M ria p e R tn e m e c a lp e R tn e m h s ib ru fe R y g re n e la n o ita re p Oe s u re ta w la n o ita re p Oe s u n o itc u rts n o c -e Dn o itilo m e d tro p s n a rT g n is s e c o rp e ts a W la s o p s iD -e s u e R-y re v o c e R-g n ilc y c e Rla itn e to p
A1 A2 A3 A4 A5 B1 B2 B3 B4 B5 B6 B7 C1 C2 C3 C4 D
X X X X X MND MND MNR MNR MNR X MND X X X X X
RESULTS OF THE LCA - ENVIRONMENTAL IMPACT according to EN 15804+A2: 1 exit device
Parameter Unit A1-A3 A4 A5 B6 C1 C2 C3 C4 D
GWP-total kg CO 2 eq 5.15E+01 1.97E+00 9.89E-01 1.75E+02 0 4.9E-02 3.2E-02 9E-03 -2.77E+01
GWP-fossil kg CO 2 eq 5.25E+01 1.9E+00 2.5E-02 1.75E+02 0 4.7E-02 3.2E-02 9E-03 -2.78E+01
GWP-biogenic kg CO 2 eq -1.03E+00 7E-02 9.64E-01 3.8E-02 0 2E-03 7.39E-07 3.16E-05 1.09E-01
GWP-luluc kg CO 2 eq 7.61E-02 4.4E-05 1.63E-05 5.3E-02 0 1.12E-06 1.79E-06 2.66E-05 -4.6E-02
ODP kg CFC11 eq 2.29E-11 1.97E-16 1.78E-16 6.17E-13 0 4.98E-18 1.6E-17 3.42E-17 -3.41E-13
AP mol H+ eq 2.83E-01 1.6E-02 2.77E-04 2.84E-01 0 4.73E-05 5.65E-06 6.62E-05 -1.14E-01
EP-freshwater kg P eq 8.49E-05 4.12E-07 3.49E-08 9.57E-05 0 1.01E-08 2.55E-09 1.59E-08 -2.43E-05
EP-marine kg N eq 4.5E-02 4E-03 1E-04 6.1E-02 0 1.5E-05 1.27E-06 1.71E-05 -1.8E-02
EP-terrestrial mol N eq 4.79E-01 4.7E-02 1E-03 6.52E-01 0 1.67E-04 2.57E-05 1.87E-04 -1.96E-01
kg NMVOC
POCP 1.33E-01 1.2E-02 2.65E-04 1.73E-01 0 4.25E-05 3.52E-06 5.16E-05 -5.6E-02
eq
ADPE kg Sb eq 3.13E-03 5.54E-08 2.82E-09 3.49E-05 0 1.42E-09 2.19E-10 8.29E-10 -8.62E-04
ADPF MJ 6.58E+02 2.62E+01 3.12E-01 2.84E+03 0 6.7E-01 1.5E-02 1.21E-01 -3.25E+02
m3 world eq
WDP 1.51E+01 4E-03 1.23E-01 3.39E+01 0 9.25E-05 3E-03 9.68E-04 -9.89E+00
deprived
GWP = Global warming potential; ODP = Depletion potential of the stratospheric ozone layer; AP = Acidification potential of land and water; EP =
Eutrophication potential; POCP = Formation potential of tropospheric ozone photochemical oxidants; ADPE = Abiotic depletion potential for non-fossil
resources; ADPF = Abiotic depletion potential for fossil resources; WDP = Water (user) deprivation potential)
RESULTS OF THE LCA - INDICATORS TO DESCRIBE RESOURCE USE according to EN 15804+A2: 1 exit device
Parameter Unit A1-A3 A4 A5 B6 C1 C2 C3 C4 D
PERE MJ 1.36E+02 8.3E-02 8.43E+00 4.49E+02 0 2E-03 3.6E-01 1.6E-02 -5.92E+01
PERM MJ 8.73E+00 0 -8.37E+00 0 0 0 -3.56E-01 0 0
PERT MJ 1.45E+02 8.3E-02 5.7E-02 4.49E+02 0 2E-03 4E-03 1.6E-02 -5.92E+01
PENRE MJ 6.59E+02 2.62E+01 3.12E-01 2.84E+03 0 6.7E-01 3.7E-01 1.21E-01 -3.26E+02
PENRM MJ 3.55E-01 0 0 0 0 0 -3.55E-01 0 0
PENRT MJ 6.59E+02 2.62E+01 3.12E-01 2.84E+03 0 6.7E-01 1.5E-02 1.21E-01 -3.26E+02
SM kg 5.53E+00 0 0 0 0 0 0 0 0
RSF MJ 0 0 0 0 0 0 0 0 0
NRSF MJ 0 0 0 0 0 0 0 0 0
FW m3 5.46E-01 1.5E-04 3E-03 1.04E+00 0 3.79E-06 7.76E-05 3.06E-05 -3.84E-01
PERE = Use of renewable primary energy excluding renewable primary energy resources used as raw materials; PERM = Use of renewable primary
energy resources used as raw materials; PERT = Total use of renewable primary energy resources; PENRE = Use of non-renewable primary energy
excluding non-renewable primary energy resources used as raw materials; PENRM = Use of non-renewable primary energy resources used as raw
materials; PENRT = Total use of non-renewable primary energy resources; SM = Use of secondary material; RSF = Use of renewable secondary fuels;
NRSF = Use of non-renewable secondary fuels; FW = Use of net fresh water
RESULTS OF THE LCA – WASTE CATEGORIES AND OUTPUT FLOWS according to EN 15804+A2:
1 exit device
Parameter Unit A1-A3 A4 A5 B6 C1 C2 C3 C4 D
HWD kg 3.04E-06 2.55E-09 4.6E-10 1.09E-06 0 6.5E-11 5.61E-11 1.85E-09 -4.77E-06
NHWD kg 4.09E+00 3E-03 3.1E-02 8.81E-01 0 6.85E-05 3E-03 6.09E-01 -1.84E+00
RWD kg 1.31E-02 2.83E-05 1.64E-05 2.53E-01 0 7.19E-07 5.46E-07 1.38E-06 -2E-03
CRU kg 0 0 0 0 0 0 0 0 0
MFR kg 0 0 0 0 0 0 1.07E+01 0 0
MER kg 0 0 0 0 0 0 0 0 0
4 Environmental Product Declaration - dormakaba - Precision 2000 Series
EEE MJ 0 0 1.5E+00 0 0 0 0 0 0
EET MJ 0 0 2.71E+00 0 0 0 0 0 0
HWD = Hazardous waste disposed; NHWD = Non-hazardous waste disposed; RWD = Radioactive waste disposed; CRU = Components for re-use;
MFR = Materials for recycling; MER = Materials for energy recovery; EEE = Exported electrical energy; EET = Exported thermal energy
RESULTS OF THE LCA – additional impact categories according to EN 15804+A2-optional:
1 exit device
Parameter Unit A1-A3 A4 A5 B6 C1 C2 C3 C4 D
Disease
PM 4.31E-06 2.56E-07 1.53E-09 2.54E-06 0 2.48E-10 7.21E-11 8.2E-10 -2.25E-06
incidence
IR kBq U235 eq 1.49E+00 4E-03 3E-03 2.09E+01 0 1.03E-04 4.92E-05 1.42E-04 -2.1E-01
ETP-fw CTUe 3.35E+02 1.85E+01 1.48E-01 8.46E+02 0 4.75E-01 6E-03 6.9E-02 -1.52E+02
HTP-c CTUh 7.39E-06 3.49E-10 7.84E-12 1.82E-08 0 8.93E-12 4.78E-13 1.03E-11 -4.39E-08
HTP-nc CTUh 1E-06 1.52E-08 3.4E-10 6.88E-07 0 3.82E-10 4.84E-11 1.13E-09 2.05E-07
SQP SQP 2.48E+02 6.8E-02 8.3E-02 2.59E+02 0 2E-03 4E-03 2.5E-02 -4.01E+01
PM = Potential incidence of disease due to PM emissions; IR = Potential Human exposure efficiency relative to U235; ETP-fw = Potential comparative
Toxic Unit for ecosystems; HTP-c = Potential comparative Toxic Unit for humans (cancerogenic); HTP-nc = Potential comparative Toxic Unit for humans
(not cancerogenic); SQP = Potential soil quality index
Disclaimer 1 – for the indicator “Potential Human exposure efficiency relative to U235”. This impact category deals mainly with the
eventual impact of low-dose ionizing radiation on human health of the nuclear fuel cycle. It does not consider effects due to possible
nuclear accidents, occupational exposure or radioactive waste disposal in underground facilities. Potential ionizing radiation from the
soil, radon and from some construction materials is also not measured by this indicator.
Disclaimer 2 – for the indicators “abiotic depletion potential for non-fossil resources”, “abiotic depletion potential for fossil resources”,
“water (user) deprivation potential, deprivation-weighted water consumption”, “potential comparative toxic unit for ecosystems”,
“potential comparative toxic unit for humans – cancerogenic”, “Potential comparative toxic unit for humans - not cancerogenic”,
“potential soil quality index”. The results of this environmental impact indicator shall be used with care as the uncertainties on these
results are high as there is limited experience with the indicator.
References
ANSI/BHMA A156.3 GaBi
ANSI/BHMA A156.3-2014; AMERICAN NATIONAL STANDARD Sphera Solutions GmbH Gabi Software System and Database
FOR EXIT DEVICES. for Life Cycle Engineering 1992-2020 Version 10.0.0.71
University of Stuttgart Leinfelden-Echterdingen
ANSI A117.1
ANSI A117.1-2017: Accessible and Usable Buildings. GaBi ts documentation
GaBi life cycle inventory data documentation (https://www.gabi-
EN 15804 software.com/support/gabi/gabidatabase- 2020-lci-
EN 15804:2019+A2, Sustainability of construction works — documentation/).
Environmental Product Declarations — Core rules for the
product category of construction products. LCA-tool dormakaba
LCA-tool, IBU-DOR-202104-LT1-EN. Developed by Sphera
REACH Solutions GmbH
Registration, Evaluation, Authorisation and Restriction of
Chemicals (REACH), Regulation (EC) No 1907/2006. Miami-Dade County Code
https://www.miamidade.gov/cob/ordinances-enacted-by-
Further References bcc.asp.
PCR Part A
BAA PCR – Part A: Calculation Rules for the Life Cycle Assessment
Buy American Act, https://www.gao.gov/products/105519. and Requirements on the Project Re-port according to EN
15804+A2:2019, Version 1.0, 2020, Institut Bauen und Umwelt
alifornia State Fire Marshal e.V., www.ibu-epd.com.
https://osfm.fire.ca.gov/.
PCR Part B
Florida Building Code PCR – Part B: Requirements on the EPD for Building Hardware
https://floridabuilding.org/c/default.aspx. product, version 1.2, Institut Bauen und Umwelt e.V., www.ibu-
epd.com, 2017.
IBU
Institut Bauen und Umwelt e.V.: General Instructions for the TAA
EPDs programme of Institut Bauen und Umwelt e.V. Version Trade Agreements Act,
2.0., Berlin: Institut Bauen und Umwelt e.V., 2021. www.ibu- https://vsc.gsa.gov/administration/compDetails.cfm.
epd.com.
UL
Illinois Accessibility Code Underwriters Laboratories,
https://www2.illinois.gov/cdb/business/codes/ https://www.ul.com/.
IllinoisAccessibilityCode/Pages/default.aspx.
5 Environmental Product Declaration - dormakaba - Precision 2000 Series
ULC
Underwriters Laboratories of Canada,
https://canada.ul.com/.
6 Environmental Product Declaration - dormakaba - Precision 2000 Series
Publisher
Institut Bauen und Umwelt e.V. +49 (0)30 3087748- 0
Hegelplatz 1 info@ibu-epd.com
10117 Berlin www.ibu-epd.com
Germany
Programme holder
Institut Bauen und Umwelt e.V. +49 (0)30 3087748- 0
Hegelplatz 1 info@ibu-epd.com
10117 Berlin www.ibu-epd.com
Germany
Author of the Life Cycle Assessment
Sphera Solutions GmbH +49 711 341817-0
Hauptstraße 111- 113 info@sphera.com
70771 Leinfelden-Echterdingen www.sphera.com
Germany
Owner of the Declaration
dormakaba International Holding GmbH +49 2333 793-0
DORMA Platz 1 info.de@dormakaba.com
58256 Ennepetal www.dormakaba.com
Germany
7 Environmental Product Declaration - dormakaba - Precision 2000 Series
