ENVIRONMENTAL PRODUCT DECLARATION
as per ISO 14025 and EN 15804+A1
Owner of the Declaration thomas gruppe - Geschäftsfeld Betonbauteile
Programme holder Institut Bauen und Umwelt e.V. (IBU)
Publisher Institut Bauen und Umwelt e.V. (IBU)
Declaration number EPD-THO-20200144-IBD1-EN
Issue date 24.08.2020
Valid to 23.08.2025
Wall elements
thomas betonbauteile
www.ibu-epd.com | https://epd-online.com
Umwelt Produktdeklaration Name des Herstellers – Name des Produkts
1. General Information
thomas betonbauteile Wall elements
Programme holder Owner of the declaration
IBU – Institut Bauen und Umwelt e.V. thomas gruppe - Geschäftsfeld Betonbauteile
Panoramastr. 1
10178 Berlin thomas beteiligungen GmbH
Germany Im Industriepark 13
55469 Simmern
Declaration number Declared product / declared unit
EPD-THO-20200144-IBD1-EN 1 t wall elements
This declaration is based on the product Scope:
category rules: This document refers to wall elements of the concrete
Pre-cast concrete components, 07.2014 components business area of the thomas group,
(PCR checked and approved by the SVR) produced in 1 out of 29 locatios:
Issue date thomas betonbauteile Rostock GmbH
24.08.2020 Werkstr. 8
18069 Rostock
Valid to
23.08.2025 The declared unit is 1 t of wall elements. The data for
the production of the declared product was collected
on a plant-specific basis with current annual data from
2018. The declarant is responsible for the underlying
data and their verification.
The owner of the declaration shall be liable for the
underlying information and evidence; the IBU shall not
be liable with respect to manufacturer information, life
cycle assessment data and evidences.
The EPD was created according to the specifications
of EN 15804+A1. In the following, the standard will be
simplified as EN 15804.
Verification
The standard EN 15804 serves as the core PCR
Independent verification of the declaration and data
according to ISO 14025:2010
Dipl. Ing. Hans Peters internally x externally
(chairman of Institut Bauen und Umwelt e.V.)
Dr. Alexander Röder Angela Schindler
(Managing Director Institut Bauen und Umwelt e.V.)) (Independent verifier appointed by SVR)
2. Product
2.1 Product description/Product definition Please format only the short name as reference and
Prefabricated walls are manufactured in the automatic the CE-marking. For the application and use the
circulation systems of the precasted concrete plants. respective national provisions apply.
Prefabricated walls consist of prefabricated reinforced
concrete slabs and are supplemented by in-situ 2.2 Application
concrete. They are used as solid walls or external Wall elements of the thomas group from the concrete
walls in the prefabricated building. The walls differ in components business area are used in prefabricated
their sizes and dimensions. buildings.They are used as
basement and storey walls in residential buildings, as
For the placing on the market of the product in the solid walls, external walls or retaining walls and
European Union/European Free Trade Association partition walls or as walls for silo buildings and water
(EU/EFTA) (with the exception of Switzerland) tanks in agricultural and industrial construction.
Regulation (EU) No. 305/2011 (CPR) applies. The
product needs a declaration of performance taking into 2.3 Technical Data
consideration EN 14992, 2012, Precast concrete The following technical data apply to wall elements.
products - wall elements and the CE-marking. The standard EN 14992 applies.
2 Environmental Product Declaration thomas gruppe – wall elements
The preliminary products such as aggregates, cement
Constructional data and reinforced steel for wall elements are delivered.
Name Value Unit The concrete is mixed together according to
Concrete Compressive predefined recipes. Before casting the wall elements,
fck ≥ C30/37 MPa
Strength the formwork is created with the desired dimensions.
Tensile strength The reinforcing bars for the reinforced concrete slabs
ftk = 550 N/mm2
reinforcing steel are attached and then filled with concrete.
Prestressing steel stress fpk N/mm2
Yield strength of Curing and Outplacement
fyk = 500 N/mm²
reinforcing steel The wall elements are cured for 8-10 hours in drying
0.1% yield strength chambers. After curing, they can be removed and can
Fp0,1 k = 595 MPa N/mm²
prestressing steel be loaded. The standard strength is reached after 28
measurement days after production.
specification,
Mechanical consistence harmonized acc. to 2.7 Environment and health during
EN 14992 manufacturing
measurement Throughout the manufacturing process, additional
Fire resistance (for the specification, measures for health safety - exceeding the legal
load capacity) harmonized acc. to measures for occupational safety for business
EN 14992 enterprises - are not required.
Hazards to water, air and soil can be excluded if the
measurement
product is used as intended. Corresponding to the
specification,
Corrsosion resistance intended use of the construction products, no health
harmonized acc. to
impairments are known due to the raw materials
EN 14992
used.At the manufacturing location, certificates of the
Gross density 2.577 t/m³
environmental management systems EN 14001 exist.
2.8 Product processing/Installation
Performance data of the product in accordance with
For the installation, the generally valid laying
the declaration of performance with respect to its
instructions of the Fachvereinigung Betonbauteile mit
essential characteristics according to EN 14992,
Gitterträgern (Association for concrete components
2012, Precast concrete products - wall elements.
with lattice girders) for wall elements must be
observed. Wall elements are unloaded from the truck
2.4 Delivery status
with the construction site crane or mobile crane and
For safety reasons and to avoid damage during
laid within the same operation.
transport wall elements can be loaded on pallets. The
dimensions of the prefabricated ceilings are:
2.9 Packaging
Wall elements are stacked and ransported to the
 Width: up to 3 m
construction site by truck. For protection against
 Length up to 9,5 m
damanges, stacking wood is placed between the
 Thickness: up to 36,5 cm panels.
2.10 Condition of use
2.5 Base materials/Ancillary materials
The wall elements are durable construction materials.
The main constituents of wall elements are:
The material composition does not change during
service life.
 Cement: < 15 M.-%
 Ingredients: < 75 M.-%
2.11 Environment and health during use
 Steel: < 6 M.-% There are no known interactions between the product,
 Water: 6 M.-% the environment and health. Hazards for air and soil
can be excluded if the described products are used as
intended.
This product or at least one partial article contains
substances listed in the candidate list (27.06.2018)
2.12 Reference service life
exceeding 0.1 percentage by mass: no.
Based on the useful lives of building components
according to the Sustainable Building Assessment
This product or at least one partial article contains
System BBSR, Service Lives of components for life
other CMR substances in categories 1A or 1B which
cycle assessment according to Assessment System for
are not on the ECHA candidate list, exceeding 0.1
Sustainable Building (BNB), the reference service life
percentage by mass: no.
of metal ceilings exceeds 50 years.
Biocide products were added to this construction
product or it has been treated with biocide products
2.13 Extraordinary effects
(this then concerns a treated product as defined by the
(EU) Ordinance on Biocide Products No. 528/2012):
Fire
no.
Wall elements declared here correspond to the class
A1 of building products regarding their fire
2.6 Manufacture
performance, according to EN 13501-1.
Shaping
Fire protection
3 Environmental Product Declaration thomas gruppe – wall elements
Name Value companies. Wall eleements can be refurbished to new
Building material class A1 building products with comparatively little effort and
Burning droplets - energy.
Smoke gas development -
2.15 Disposal
Water Remains of wall elements and those from demolition
There are no known effects on the environment in the occurring on the construction site, can be disposed of
event of unforeseen ingress of water. in accordance with the local regulations or Waste
Classification Ordinance (AVV) and the European
Mechanical destruction Waste Catalogue (EWC). The disposal code is 17 01
In the case of mechanical destruction, wall elements 01 (concrete), if the recycling options mentioned above
may break. are not practical.
2.14 Re-use phase 2.16 Further information
Individual components of wall elements, such as Processing instructions, product data sheets, safety
concrete and steel, can be re-used after varietal information and other technical information are
segregation. Concrete can be ground and used as an available for download on the website of the thomas
additive in the production of building materials as a group:
secondary raw material input, e.g. as filler and fill www.thomas-gruppe.de
material in civil engineering, road construction or e.g.
for noise barriers.
The steel scrap is collected and sent either directly or
via the scrap metal trade to secondary smelting
3. LCA: Calculation rules
3.1 Declared Unit data regarding transport distances were suplemented
The declaration applies to 1 t of wall elements. by estimates based on a medium transport distance of
Wall elements vary in volume, mass and slightly in 300 km in Germany.
composition. The average calculation is based on the
average annual production. 3.4 Cut-off criteria
All relevant data, i.e. all applied materials according to
Declared unit the recipe and the energy used originate from the
Name Value Unit production data acquisition and have been considered
Declared unit 1 t within the inventory analysis. Material- and
Grammage 0.142 t/m² energyflows with a proportion of less than 1 % were
Density 2577 t/m³ collected. It can be assumed, that the sum of the
Conversion factor to 1 kg 0.001 - neglected processes does not exceed 5 % of the
impact categories.
3.5 Background data
3.2 System boundary Primary data has been provided by the manufacturer.
The Life Cycle Assessment considers the system All background data required for the Life Cycle
boundaries "cradle to grave" and follows the modular Assessment originates form the database
construction system described by EN 15804. The LCA ÖKOBAUDAT 2019-III. Individual flows were
takes into account the following complemented by ecoinvent 3.6 and GaBi ts 7.3.3.
modules:
3.6 Data quality
 A1: Raw material supply: extraction of raw The Life Cycle Assessment was essentially calculated
based on result from impact assessments of upstream
material, production of precursors, processing
activities. This leads to limitations on delared indicators
of cement and aggregates, steel production,
(SM) and modules C3 and D.
casting and processing of recycling materials
For modelling the Life Cycle of prefabricated
 A2: Transport of precursors: transport of raw ceilings,data has been from the production year
materials to manufacturing plant 2018.Background data has been taken from the
 A3: Manufacturing: production of wall variousdatabase. For the Life Cycle Inventory all input
and output flows have been respected.
elements
 C1: De-Construction & Demolition of wall
elements
 C2: Transportation towards disposal
 C4: Disposal of wall elements 3.7 Period under review
The amount of raw materials, input energy and the
volume of waste relate to the year 2018. It corresponds
to the best currently available technology and thus is
3.3 Estimates and assumptions
representative for the considered time period. The
Plant and process specific data was provided for the
reference area is Germany.
Life Cycle Assessment. Missing information on primary
4 Environmental Product Declaration thomas gruppe – wall elements
3.8 Allocation context, respectively the product-specific
Co-product allocation does not exist in the characteristics of performance, are taken into account.
manufacturing process.
The background data was used from various LCA
3.9 Comparability database. Thereby limitations on comparability of
Basically, a comparison or an evaluation of EPD data EPDs may result.
is only possible if all the data sets to be compared The LCA background database ÖKOBAUDAT 2019-III
were created according to EN 15804 and the building was used. Individual flows were complemented by
ecoinvent 3.6:2019 and GaBi ts 7.3.3.
4. LCA: Scenarios and additional technical information
The following technical information models the basisfor
the declared modules or can be used for developing
specific scenarios within the context of a building
assessment.
The reference life span according to ISO 15686-1
could not have been determined. The declaration of
the reference life span underlies the assessment
system of the Federal Institute for Research on
Building, Urban Affairs and Spatial Development
BBSR.
Reference service life
Name Value Unit
Reference service life (according to
- a
ISO 15686-1, -2, -7 and -8)
Life Span (according to BBSR) ≥ 50 a
End of life (C1-C4)
Name Value Unit
Landfilling 945 kg
Recycling 55 kg
5 Environmental Product Declaration thomas gruppe – wall elements
5. LCA: Results
The table displayed below summarizes the results of the Life Cycle Assessment (LCA). The results of the impact
assessment do not provide any information on endpoints of the impact categories, exceedances of thresholds,
safety margins or risks. The results refer to the declared unit of 1 t wall elements. The Impact Assessment is
based on /CML 2001/ - April 2015. The Impact Assessment is based on CML 2001 - April 2015.
DESCRIPTION OF THE SYSTEM BOUNDARY (X = INCLUDED IN LCA; MND = MODULE NOT DECLARED;
MNR = MODULE NOT RELEVANT)
BENEFITS AND
CONSTRUCTI LOADS
PRODUCT STAGE ON PROCESS USE STAGE END OF LIFE STAGE BEYOND THE
STAGE SYSTEM
BOUNDARIES
6 Environmental Product Declaration thomas gruppe – wall elements
lairetam
waR
ylppus tropsnarT
gnirutcafunaM
eht
morf
tropsnarT
etis
eht
ot
etag
ylbmessA esU
ecnanetniaM
riapeR
tnemecalpeR tnemhsibrufeR
ygrene
lanoitarepO esu
retaw
lanoitarepO esu
noitcurtsnoc-eD
noitilomed tropsnarT
gnissecorp
etsaW
lasopsiD -esueR -yrevoceR -gnilcyceR laitnetop
A1 A2 A3 A4 A5 B1 B2 B3 B4 B5 B6 B7 C1 C2 C3 C4 D
X X X MND MND MND MND MNR MNR MNR MND MND X X MND X MND
RESULTS OF THE LCA - ENVIRONMENTAL IMPACT according to EN 15804+A1: 1 t wall elements
Parameter Unit A1-A3 C1 C2 C4
Global warming potential [kg CO2-Eq.] 1.79E+2 8.63E-1 1.92E+0 1.41E+1
Depletion potential of the stratospheric ozone layer [kg CFC11-Eq.] 5.09E-7 2.84E-16 9.11E-16 8.26E-14
Acidification potential of land and water [kg SO2-Eq.] 2.24E-1 6.07E-4 4.33E-3 8.43E-2
Eutrophication potential [kg (PO4)3--Eq.] 5.02E-2 8.70E-5 1.06E-3 9.56E-3
Formation potential of tropospheric ozone photochemical
[kg ethene-Eq.] 2.58E-2 9.06E-5 -1.34E-3 6.47E-3
oxidants
Abiotic depletion potential for non-fossil resources [kg Sb-Eq.] 1.38E-4 3.02E-8 1.86E-7 5.18E-6
Abiotic depletion potential for fossil resources [MJ] 1.11E+3 1.18E+1 2.57E+1 1.97E+2
RESULTS OF THE LCA - RESOURCE USE according to EN 15804+A1: 1 t wall elements
Parameter Unit A1-A3 C1 C2 C4
Renewable primary energy as energy carrier [MJ] 3.13E+2 5.35E-2 1.61E+0 2.59E+1
Renewable primary energy resources as material utilization [MJ] 0.00E+0 0.00E+0 0.00E+0 0.00E+0
Total use of renewable primary energy resources [MJ] 3.13E+2 5.35E-2 1.61E+0 2.59E+1
Non-renewable primary energy as energy carrier [MJ] 1.23E+3 1.19E+1 2.58E+1 2.04E+2
Non-renewable primary energy as material utilization [MJ] 0.00E+0 0.00E+0 0.00E+0 0.00E+0
Total use of non-renewable primary energy resources [MJ] 1.23E+3 1.19E+1 2.58E+1 2.04E+2
Use of secondary material [kg] IND 0.00E+0 0.00E+0 0.00E+0
Use of renewable secondary fuels [MJ] 0.00E+0 0.00E+0 0.00E+0 0.00E+0
Use of non-renewable secondary fuels [MJ] 0.00E+0 0.00E+0 0.00E+0 0.00E+0
Use of net fresh water [m³] 4.37E-1 8.45E-5 1.82E-3 5.13E-2
RESULTS OF THE LCA – OUTPUT FLOWS AND WASTE CATEGORIES according to EN 15804+A1:
1 t wall elements
Parameter Unit A1-A3 C1 C2 C4
Hazardous waste disposed [kg] 3.84E-3 1.69E-9 1.46E-6 3.47E-6
Non-hazardous waste disposed [kg] 2.54E+1 1.51E-3 1.83E-3 9.47E+2
Radioactive waste disposed [kg] 4.31E-2 1.18E-5 3.90E-5 2.70E-3
Components for re-use [kg] 0.00E+0 0.00E+0 0.00E+0 0.00E+0
Materials for recycling [kg] 4.22E-1 0.00E+0 5.46E+1 0.00E+0
Materials for energy recovery [kg] 0.00E+0 0.00E+0 0.00E+0 0.00E+0
Exported electrical energy [MJ] 0.00E+0 0.00E+0 0.00E+0 0.00E+0
Exported thermal energy [MJ] 0.00E+0 0.00E+0 0.00E+0 0.00E+0
* MND: Modul not declared
6. LCA: Interpretation
The following figure shows the relative contributions of of the reinforcing steel in the product. The product
different Life Cycle processes and the primary energy considered in the model has a share of reinforcement
demand in the form of a dominance analysis. steel of 0.055 M% and has a greenhouse gas potential
(GWP) of 179 kgCO2e within production (A1–3). The
The Life Cycle Assessment was essentially calculated proportion of reinforcement can vary in individual
based on result from impact assessments of upstream cases (0.05 - 0.104 M%) and cause a range of the
activities. This leads to limitations on delared indicators greenhouse gas potential (GWP) within production
(SM) and modules C3 and D. (A1–3) of between -1 % to +15 %. Unless otherwise
Deviations in the material composition within the stated, the fluctuations in all other
product may occur. The influence on the range of the impact categories are also small (<10 %).
environmental impact is determined by the proportion
Indicators of the impact assessment Potential of tropospheric ozone photochemical
oxidants (POCP)
The impact categories are determined throughout the About 60 % of the Photochemical oxidant potential is
life cycle mostly by module A1 (raw materials). The triggered by the use of cement and by the use of steel
main driver is the use of cement, which contributes (58 %). Due to different reinforcement components in
about to 64 % to the greenhouse gas potential (GWP) the product, the POCP factor can fluctuate by -2% to +
in the production stage (A1 – A3), followed by steel 48%.
with 21 %. Contributions to the environmental impact The negative POCP value for the transports is
from the transport of the preliminary products explained by the methodical approach in calculating
(according to the assumed scenario for A2) and the the impact indicator: The negative POCP in the
energy input for production (A3) within the production transports is caused by the division of the NOX
stage are comparable small. For the disposal of the emissions into the two individual emissions NO2 and
construction waste (C1 – C4) additional environmental NO. The NO has a negative influence on the POCP, as
burden occurs. it reduces the formation of ozone near the ground.
Global warming potential (GWP) Abiotic depletion potential for non-fossil resources
The global warming potential is mainly determined with (ADP elem.)
89% by the supply of raw materials: cement accounts The ADP elem.-value is determined almost exclusively
for 64 % and steel for 21 %. The thermal energy by the provision of cement (89 %) and steel (8 %) at
requirement and use of electricity contribute with 7 % the production stage. Electricity contributes for 1 % to
to the GWP factor and the transport of preliminary the ADP elem.-factor.
products with approx. 5 %.
Abiotic depletion potential for fossil resources
Depletion potential of the stratospheric ozone layer (ADP foss.)
(ODP) Within the production stage (A1 – A3), the ADP foss.-
The Ozone depletion potential is dominated almost value results mainly from high energy consumption
exclusively by the preliminary products (approx. 100 required for the provision of cement and steel (approx.
%) and within them almost exclusively by the use of 69 % in total). The use of electricity contributes for 4
cement. The use of electricity causes 100% of the %, fuel for 8 %. The proportions of reinforcing steel in
ODP factor within manufacturing (A3). the products can vary and cause average fluctuations
in the ADP foss. faktor of (-1 % / + 31 %).
Acidification potential of land and water (AP)
The Acidification potential is determined by 45 % by Within the production (A1-3), the total primary energy
cement and 36 % by steel in the production stage. The demand is divided between approx. 80 %
use of energy sources in A3 contributes for 5 % to the nonrenewable energy sources and approx. 20 %
AP. With approx. 8 %, the transports have a minor renewable energies.
influence on the acidification potential. With different
proportions of reinforcementsteel in the product, the Total use of non-renewable primary energy
AP-factor may vary by -1 % to + 29 %. resources (PENRT)
The demand for non-renewable primary energy
Eutrophication potential (EP) resources result mainly for 80% from raw materials
The Eutrophication potential is determined by 62 % by (A1). The transport of the preliminary products (A2)
cement and with 20 % by steel in the production stage. contribute for 9 % and the production of the declared
The use of energy sources in A3 contributes for 2 % to product (A3) for 11 % to the PENRT value.
the EP. With approx. 8 %, the transports have a minor For the disposal of the construction waste additional
influence on the acidification potential. With different use of non-renewable energy is due at the end of life.
proportions of reinforcementsteel in the product, the In practice, different proportions of reinforcement are
EP-factor may vary by -1 % to + 14 %. used in the product (0.05 - 0.104 M%) and can cause
fluctuations in the non-renewable primary energy
7 Environmental Product Declaration thomas gruppe – wall elements
demand (PENRT) in the range of -1 % to + 34 % within For the disposal of the construction waste additional
the production (A1–3). use of renewable energy is due at the end of life.
Total use of renewable primary energy resources In practice, different proportions of reinforcement are
(PERT) used in the product (0.05 - 0.104 M%) and can cause
In comparison to the PENRT value the share of fluctuations in the renewable primary energy demand
renewable resources is low. The majority of the PERT (PERT) within the production (A1–3) in the range from
value is made up of raw material supply (A1) with 93 -2 % to +56 %.
%, transportation for 2 % and the energy required for
production with approx. 4 %.
7. Requisite evidence
Not relevant.
8. References
BBSR Candidate List
Federal Institute for Research on Building, Urban European Chemical Agency (ECHA): Candidate List of
Affairs and Spatial Development (BBSR): Service lifes substances of very high concern for Authorisation, in:
of construction components. Service lifes of https://echa.europa.eu/candidate-list-table, 2020.
construction components for Life Cycle Assessments
according to the assessment system for sustainable
construction (BNB), in: Federal Ministry for the CMR Substances
Environment, Nature Conservation, Building and European Chemical Agency (ECHA): CMR substances
Nuclear Safety (ed.), 2017. from Annex VI of the CLP regulation registered under
REACH and/ or notified under CLP.
Regulation 528/2012
Regulation (EU) No 528/2012 of the European ÖKOBAUDAT 2019-III
Parliament and of the Council of 22 May 2012 Federal Ministry of the Interior, Building and
concerning the making available on the market and Community (editor): Version 2019-III from 29.05.2019.
use of biocidal products, in: Official Journal of the
European Union L 161/I, 2012. PCR A
Product category rules for building-related products
Construction Product Regulation and service. Part A: Calculation rules for Life Cycle
Construction Product Regulation (CPR): Regulation Assessment and requirements on the project report,
(EU) No 305/2011 of the European Parliament and of version 1.7, 2018. Institut Bauen und Umwelt e.V.
the Council of 9 March 2011 laying down harmonised
conditions for the marketing of construction products PCR B
and repealing Council Directive 89/106/EEC (Text with PCR Guidance texts for building-related products and
EEA relevance), in: Official Journal of the European service. Part B: Requirements on the EPD for pre-cast
Union, 2011. concrete components, version 1.7, 2019. Institut
Bauen und Umwelt e.V.
CML 2001
Centrum voor Milieukunde der Universität Leiden, EN 1350-1
Institute of Environmental Sciences, Leiden University, EN13501-1: 2019, Fire classification of construction
The Netherlands: "Life Cycle Assessment. An products and building elements - Part 1: Classification
operational guide to the ISO standards, Volume 1, 2 using data from reaction to fire tests.
and 3", 2001.
EN 14992
European Waste Catalogue DIN EN 14992:2012-09, Precast concrete products -
Waste Classification Ordinance (AVV)/ European Wall elements.
Waste Catalogue (EWC): Waste Classification.
Disposal Code 17 01 01 concrete. EN 15804
EN 15804:2012-04+A1 2013, Sustainability of
ecoinvent 3.6 construction works — Environmental Product
ecoinvent V. 3.6: Databank Version 3.6, Switzerland, Declarations — Core rules for the product category of
Dübendorf, [Access on 09.04.2019]. construction products.
Fachvereinigung Betonbauteile mit Gitterträgern
Fachvereinigung Betonbauteile mit Gitterträgern e.V. ISO 14025
(Hrsg.): Verlegeanleitung Elementdecken, 2012. DIN EN ISO 14025:2011-10, Environmental labels and
declarations — Type III environmental declarations —
GaBi 7.3.3 Principles and procedures.
GaBi 7.3.3 databank edition, Thinkstep AG, 2017.
ISO 14001
8 Environmental Product Declaration thomas gruppe – wall elements
ISO 14001: Environmental management systems -
Requirements with guidance for use.
ISO15686-1
ISO 15686-1:2011-05 Buildings and constructed
assets - Service life planning - Part 1: General
principles and framewok.
9 Environmental Product Declaration thomas gruppe – wall elements
Publisher
Institut Bauen und Umwelt e.V. Tel +49 (0)30 3087748- 0
Panoramastr. 1 Fax +49 (0)30 3087748- 29
10178 Berlin Mail info@ibu-epd.com
Germany Web www.ibu-epd.com
Programme holder
Institut Bauen und Umwelt e.V. Tel +49 (0)30 - 3087748- 0
Panoramastr 1 Fax +49 (0)30 – 3087748 - 29
10178 Berlin Mail info@ibu-epd.com
Germany Web www.ibu-epd.com
Author of the Life Cycle
Assessment Tel +49 7121 9223 50
myclimate Deutschland gGmbH Fax +49 7121 9223 8050
Borsigstraße 6 Mail kontakt@myclimate.de
72760 Reutlingen Web www.myclimate.de
Germany
Owner of the Declaration
thomas gruppe - Geschäftsfeld Tel +49 (6761) 901 100
Betonbauteile Fax +49 (6761) 901 101
Im Industriepark 13 Mail info@thomas-gruppe.de
55469 Simmern Web www.thomas-gruppe.de
Germany
