ENVIRONMENTAL PRODUCT DECLARATION
as per ISO 14025 and EN 15804+A1
Owner of the Declaration Balsan
Programme holder Institut Bauen und Umwelt e.V. (IBU)
Publisher Institut Bauen und Umwelt e.V. (IBU)
Declaration number EPD-BAL-20200070-CCA1-EN
Issue date 07.05.2020
Valid to 06.05.2025
PILOTE 2
tufted carpet tiles made of recycled pile material
BALSAN
www.ibu-epd.com | https://epd-online.com
Umwelt Produktdeklaration Name des Herstellers – Name des Produkts
General Information
Balsan PILOTE 2 - tufted carpet tiles made of
recycled pile material
Programme holder Owner of the declaration
IBU – Institut Bauen und Umwelt e.V. Balsan
Panoramastr. 1 Corbilly - D14
10178 Berlin 36330 Arthon
Germany France
Declaration number Declared product / declared unit
EPD-BAL-20200070-CCA1-EN 1 m² tufted carpet tiles PILOTE 2
This declaration is based on the product Scope:
category rules: The manufacturer declaration applies to the tufted
Floor coverings, 02/2018 carpet tiles PILOTE 2.
(PCR checked and approved by the SVR) The products are produced in the Balsan
manufacturing sites Arthon (tufting and precoating) and
Issue date Neuvy-Saint-Sépulchre, France (back coating).
07.05.2020 The declaration is only valid in conjunction with a valid
GUT-PRODIS license of the product.
Valid to
06.05.2025 The owner of the declaration shall be liable for the
underlying information and evidence; the IBU shall not
be liable with respect to manufacturer information, life
cycle assessment data and evidences.
The EPD was created according to the specifications
of EN 15804+A1. In the following, the standard will be
simplified as EN 15804.
Verification
The standard EN 15804 serves as the core PCR
Independent verification of the declaration and data
according to ISO 14025:2010
Dipl. Ing. Hans Peters internally x externally
(chairman of Institut Bauen und Umwelt e.V.)
Dr. Alexander Röder Angela Schindler
(Managing Director Institut Bauen und Umwelt e.V.)) (Independent verifier appointed by SVR)
Product
Product description/Product definition Application
PILOTE 2 - tufted carpet tiles having a surface pile of According to the use class as defined in EN 1307 the
solution-dyed polyamide 6 with 100% recycled content, products can be used in all professional areas which
a polyester primary backing with 90% recycled content require class 33 or less.
and a bitumen based heavy backing with a fibre glass
reinforcement and a polyester fleece backing.
The recycled content amounts to 16%.
For the placing on the market of the product in the
Technical Data
European Union/European Free Trade Association
The performance data listed in the DoP apply.
(EU/EFTA) (with the exception of Switzerland)
Regulation (EU) No. 305/2011 Construction Product
Regulation (CPR) applies. The product needs a
Name Value Unit
Declaration of Performance (DoP) taking into
Product Form Tiles 50 cm x 50 cm -
consideration EN 14041 and the CE-marking. The DoP
Type of manufacture Tufted tiles -
of the product can be found on the manufacturer's
Yarn type Polyamide 6, 100 % recycled -
technical information section. For the application and
Secondary backing Bitumen based heavy backing -
use of the product the respective national provisions
Total pile weight 580 g/m²
apply.
Surface pile weight 350 g/m2
Total carpet weight 4200 g/m2
2 Environmental Product Declaration Balsan – PILOTE² - tufted carpet tiles
The products are registered in the GUT-PRODIS
Information System. The PRODIS system ensures the
Performance data of the product in accordance with compliance with limitations of various chemicals and
the declaration of performance with respect to its Volatile Organic Compound (VOC)-emissions and a
essential characteristics according to EN 14041. ban on the use of all substances that are listed as
Additional product properties in accordance with EN 'Substances of Very High Concern' (SVHC) under
1307 can be found on the Product Information System REACH.
PRODIS using the PRODIS registration number of the This product contains substances listed in the Reach
product (www.pro-dis.info) or on the manufacturer's candidate list (27.06.2018) exceeding 0.1 percentage
technical information section (www.balsan.com). by mass: no
Base materials/Ancillary materials Reference service life
A calculation of the reference service life according to
Name Value Unit ISO 15686 is not possible.
Polyamide 6 13.8 % The service life of textile floor coverings strongly
Polyester 4.3 % depends on the correct installation taking into account
SBR-latex 3.5 % the declared use classification and the adherence to
Mineral filler 60.8 % cleaning and maintenance instructions.
Bitumen 16.7 % A minimum service life of 10 years can be
Glass fibre 0.8 % assumed, technical service life can be considerably
Additives 0.1 % longer.
LCA: Calculation rules
Declared Unit occurs as installation waste including its transport to
the place of installation.
Generated electricity and steam due to the incineration
Name Value Unit of waste are listed in the result table as exported
Declared unit 1 m2 energy.
Mass reference 4,20 kg/m² Preparation of the floor and auxiliary materials
The declared unit refers to 1 m2 produced textile floor (adhesives, fixing agents, PET connectors) are beyond
covering. The output of module A5 'Assembly' is 1 m2 the system boundaries and not taken into account.
installed textile floor covering.
B1 Use:
Indoor emissions during the use stage. After the first
year, no product-related Volatile Organic Compound
System boundary (VOC) emissions are relevant due to known VOC
decay curves of the product.
Type of EPD: Cradle-to-grave
B2 Maintenance:
System boundaries of modules A, B, C, D: Cleaning of the textile floor covering for a period of 1
Modules C3, C4 and D are indicated separately for year:
three end-of-life scenarios: Vacuum cleaning – electricity supply
1 - landfill disposal Wet cleaning – electricity, water consumption,
2 - municipal waste incineration production of the cleaning agent, waste water
3 - recovery in a cement plant treatment.
The declared values in this module have to be
A1-A3 Production: multiplied by the assumed service life of the floor
Energy supply and production of the basic material, covering in the building in question.
processing of secondary material, auxiliary material,
transport of the material to the manufacturing site, B3 - B7:
emissions, waste water treatment, packaging material The modules are not relevant and therefore not
and waste processing up to the landfill disposal of declared.
residual waste (except radioactive waste). Benefits for
generated electricity and steam due to the incineration C1 De-construction:
of production waste are aggregated. The floor covering is de-constructed manually and no
additional environmental impact is caused.
A4 Transport:
Transport of the packed textile floor covering C2 Transport:
from factory gate to the place of installation. Transport of the carpet waste to a landfill, to the
municipal waste incineration plant (MWI) or to the
A5 Installation: waste collection facility for recycling.
Installation of the textile floor covering, processing of
installation waste and packaging waste up to the C3 Waste processing:
landfill disposal of residual waste (except radioactive C3-1: Landfill disposal needs no waste processing.
waste), the production of the amount of carpet that C3-2: Impact from waste incineration (plant with
3 Environmental Product Declaration Balsan – PILOTE² - tufted carpet tiles
R1>0.6), generated electricity and steam are listed in D-2: Benefits for generated energy due to incineration
the result table as exported energy. of carpet waste at the end-of-life (incineration plant
C3-3: Collection of the carpet waste, waste processing with R1 > 0.6),
(granulating). D-3: Benefits for saved fossil energy and saved
inorganic material due to recovery of the carpet in a
C4 Disposal cement plant at the end-of-life, transport from the
C4-1: Impact from landfill disposal, reprocessing plant to the cement kiln.
C4-2: The carpet waste leaves the system in
module C3-2, Comparability
C4-3: The pre-processed carpet waste leaves the Basically, a comparison or an evaluation of EPD data
system in module C3-3. is only possible if all the data sets to be compared
were created according to EN 15804 and the building
D Recycling potential: context, respectively the product-specific
Calculated benefits result from materials exclusive characteristics of performance, are taken into account.
secondary materials (net materials).
D-A5: Benefits for generated energy due Background data are taken from the GaBi database
to incineration of packaging and installation waste 2020, service pack 40. Remaining data gaps are
(incineration plant with R1 > 0.6), covered by the ecoinvent 3.6 database.
D-1: Benefits for generated energy due to landfill
disposal of carpet waste at the end-of-life,
LCA: Scenarios and additional technical information
The following information refer to the declared modules End of Life (C1-C4)
and are the basis for calculations or can be used for Three different end-of-life scenarios are declared and
further calculations. the results are indicated separately in module C.
Each scenario is calculated as a 100% scenario.
Transport to the construction site (A4) Scenario 1: 100% landfill disposal
Name Value Unit Scenario 2: 100% municipal waste incineration (MWI)
Litres of fuel (truck, EURO 0-6 mix) 0.03 l/100km with R1>0.6
Transport distance 700 km Scenario 3: 100% recycling in the cement industry
Capacity utilisation (including empty
55 %
runs) If combinations of these scenarios have to be
Gross density of products transported 725 kg/m3 calculated this should be done according to the
following scheme:
Installation in the building (A5) EOL-impact = x% impact (Scenario 1)
Name Value Unit + y% impact (Scenario 2)
Material loss 0.13 kg + z% impact (Scenario 3)
Polyethylene packaging waste and installation waste with x% + y% + z% = 100%
are considered to be incinerated in a municipal waste
incineration plant. Cardboard is going to be recycled. Name Value Unit
Preparation of the floor and auxiliaries (adhesives, Collected as mixed construction waste 4.2 kg
fixing agents, PET connectors etc.) are not taken into (scenario 1 and 2)
account. Collected separately (scenario 3) 4.2 kg
Landfilling (scenario 1) 4.2 kg
Maintenance (B2) Energy recovery (scenario 2) 4.2 kg
The values for cleaning refer to 1 m2 floor covering Energy recovery (scenario 3) 1.61 kg
used in commercial areas per year. Recycling (scenario 3) 2.59 kg
Depending on the application based on ISO 10874, the
technical service life recommended by the Reuse, recovery and/or recycling potentials (D),
manufacturer and the anticipated strain on the floor by relevant scenario information
customers, the case-specific useful life can be Recovery or recycling potentials due to the three end-
established. The effects of Module B2 need to be of-life scenarios (module C) are indicated separately.
calculated based on the useful life to obtain the overall Recycling in the cement industry (scenario 3)
environmental impacts. The organic material of the carpet is used as
Name Value Unit secondary fuel in a cement kiln. It mainly substitutes
Maintenance cycle (wet cleaning) 1.5 1/year for lignite (64.5%), hard coal (26.5%) and petrol coke
Maintenance cycle (vacuum (9.0%) VDZ e.V.
208 1/year
cleaning) The inorganic material is substantially integrated into
Water consumption (wet cleaning) 0.004 m3 the cement clinker and substitutes for original material
Cleaning agent (wet cleaning) 0.09 kg input.
Electricity consumption 0.314 kWh
Further information on cleaning and maintenance see
www.balsan.com
4 Environmental Product Declaration Balsan – PILOTE² - tufted carpet tiles
LCA: Results
The declared result figures in module B2 have to be multiplied by the assumed service life (in years) of the floor
covering in the building under consideration.
Information on un-declared modules:
Modules B3 - B7 are not relevant during the service life of the carpet and are therefore not declared.
Modules C1, C3/1, C4/2 and C4/3 cause no additional impact (see "LCA: Calculation rules") and are therefore not
declared. Module C2 represents the transport for scenarios 1, 2 and 3. Column D represents module D/A5.
The CML characterisation factors version January 2016 are applied.
DESCRIPTION OF THE SYSTEM BOUNDARY (X = INCLUDED IN LCA; MND = MODULE NOT DECLARED;
MNR = MODULE NOT RELEVANT)
BENEFITS AND
CONSTRUCTI LOADS
PRODUCT STAGE ON PROCESS USE STAGE END OF LIFE STAGE BEYOND THE
STAGE SYSTEM
BOUNDARIES
5 Environmental Product Declaration Balsan – PILOTE² - tufted carpet tiles
lairetam
waR
ylppus tropsnarT
gnirutcafunaM
eht
morf
tropsnarT
etis
eht
ot
etag
ylbmessA esU
ecnanetniaM
riapeR
tnemecalpeR tnemhsibrufeR
ygrene
lanoitarepO esu
retaw
lanoitarepO esu
noitcurtsnoc-eD
noitilomed tropsnarT
gnissecorp
etsaW
lasopsiD -esueR -yrevoceR -gnilcyceR laitnetop
A1 A2 A3 A4 A5 B1 B2 B3 B4 B5 B6 B7 C1 C2 C3 C4 D
X X X X X X X MNR MNR MNR MND MND MND X X X X
RESULTS OF THE LCA - ENVIRONMENTAL IMPACT according to EN 15804+A1: 1 m² floorcovering
Parameter Unit A1-A3 A4 A5 B1 B2 C2 C3/2 C3/3 C4/1 D D/1 D/2 D/3
GWP [kg CO2-Eq.] 3.90E+0 2.49E-1 3.30E-1 0.00E+0 2.92E-1 1.39E-2 5.74E+0 2.31E-2 2.82E-1 -3.61E-2 0.00E+0-1.15E+0-1.91E-1
-5.00E- -1.60E- -9.70E-
ODP [kg CFC11-Eq.] 8.39E-9 4.08E-172.52E-100.00E+0 1.21E-8 2.28E-181.78E-156.89E-169.18E-16 0.00E+0
16 14 16
AP [kg SO2-Eq.] 8.74E-3 1.05E-3 3.62E-4 0.00E+0 1.16E-3 5.86E-5 2.20E-3 4.83E-5 7.68E-4 -4.49E-5 0.00E+0 -1.43E-3 -6.10E-4
EP [kg (PO4)3--Eq.] 1.84E-3 2.63E-4 7.99E-5 0.00E+0 3.17E-4 1.47E-5 5.37E-4 5.35E-6 8.03E-4 -5.62E-6 0.00E+0 -1.79E-4 -6.93E-5
POCP [kg ethene-Eq.] 6.84E-4 -4.42E-4 1.06E-5 6.29E-5 1.48E-4 -2.47E-5 1.44E-4 3.44E-6 8.67E-5 -4.12E-6 0.00E+0 -1.32E-4 -1.50E-4
ADPE [kg Sb-Eq.] 4.44E-6 2.10E-8 1.39E-7 0.00E+0 4.43E-6 1.17E-9 1.68E-7 7.71E-9 5.48E-8 -6.65E-9 0.00E+0 -2.12E-7 -2.11E-8
ADPF [MJ] 8.82E+1 3.39E+0 2.83E+0 0.00E+0 6.76E+0 1.89E-1 2.46E+0 2.55E-1 4.22E+0 -5.07E-1 0.00E+0-1.62E+1-3.22E+1
GWP = Global warming potential; ODP = Depletion potential of the stratospheric ozone layer; AP = Acidification potential of land and water; EP =
Caption Eutrophication potential; POCP = Formation potential of tropospheric ozone photochemical oxidants; ADPE = Abiotic depletion potential for non-
fossil resources; ADPF = Abiotic depletion potential for fossil resources
RESULTS OF THE LCA - RESOURCE USE according to EN 15804+A1: 1 m² floorcovering
Parameter Unit A1-A3 A4 A5 B1 B2 C2 C3/2 C3/3 C4/1 D D/1 D/2 D/3
PERE [MJ] 2.73E+1 1.91E-1 8.39E-1 0.00E+0 1.20E+0 1.07E-2 4.21E-1 1.83E-1 3.06E-1 -1.33E-1 0.00E+0 -4.25E+0 -2.11E-1
PERM [MJ] 0.00E+0 0.00E+0 0.00E+0 0.00E+0 0.00E+0 0.00E+0 0.00E+0 0.00E+0 0.00E+0 0.00E+0 0.00E+0 0.00E+0 0.00E+0
PERT [MJ] 2.73E+1 1.91E-1 8.39E-1 0.00E+0 1.20E+0 1.07E-2 4.21E-1 1.83E-1 3.06E-1 -1.33E-1 0.00E+0 -4.25E+0 -2.11E-1
PENRE [MJ] 6.01E+1 3.40E+0 3.09E+0 0.00E+0 7.86E+0 1.90E-1 3.92E+1 3.68E+1 4.36E+0 -6.22E-1 0.00E+0 -1.99E+1 -3.23E+1
PENRM [MJ] 3.64E+1 0.00E+0 0.00E+0 0.00E+0 0.00E+0 0.00E+0 -3.64E+1 -3.64E+1 0.00E+0 0.00E+0 0.00E+0 0.00E+0 0.00E+0
PENRT [MJ] 9.65E+1 3.40E+0 3.09E+0 0.00E+0 7.86E+0 1.90E-1 2.76E+0 4.13E-1 4.36E+0 -6.22E-1 0.00E+0 -1.99E+1 -3.23E+1
SM [kg] 7.91E-1 0.00E+0 2.37E-2 0.00E+0 0.00E+0 0.00E+0 0.00E+0 0.00E+0 0.00E+0 0.00E+0 0.00E+0 0.00E+0 2.59E+0
RSF [MJ] 0.00E+0 0.00E+0 0.00E+0 0.00E+0 0.00E+0 0.00E+0 0.00E+0 0.00E+0 0.00E+0 0.00E+0 0.00E+0 0.00E+0 0.00E+0
NRSF [MJ] 0.00E+0 0.00E+0 0.00E+0 0.00E+0 0.00E+0 0.00E+0 0.00E+0 0.00E+0 0.00E+0 0.00E+0 0.00E+0 0.00E+0 3.64E+1
FW [m³] 8.55E-2 2.21E-4 3.09E-3 0.00E+0 4.27E-3 1.24E-5 1.70E-2 2.12E-4 5.35E-5 -1.54E-4 0.00E+0 -4.92E-3 -2.64E-3
PERE = Use of renewable primary energy excluding renewable primary energy resources used as raw materials; PERM = Use of
renewable primary energy resources used as raw materials; PERT = Total use of renewable primary energy resources; PENRE = Use of
non-renewable primary energy excluding non-renewable primary energy resources used as raw materials; PENRM = Use of non-
Caption
renewable primary energy resources used as raw materials; PENRT = Total use of non-renewable primary energy resources; SM = Use
of secondary material; RSF = Use of renewable secondary fuels; NRSF = Use of non-renewable secondary fuels; FW = Use of net fresh
water
RESULTS OF THE LCA – OUTPUT FLOWS AND WASTE CATEGORIES according to EN 15804+A1:
1 m² floorcovering
Parameter Unit A1-A3 A4 A5 B1 B2 C2 C3/2 C3/3 C4/1 D D/1 D/2 D/3
HWD [kg] 2.70E-3 1.58E-7 8.11E-5 0.00E+0 9.63E-10 8.84E-9 2.13E-8 1.71E-10 1.59E-8 -2.48E-10 0.00E+0 -7.91E-9 1.26E-8
NHWD [kg] 6.63E-1 5.20E-4 5.56E-2 0.00E+0 5.63E-3 2.91E-5 1.19E+0 2.93E-4 4.18E+0 -2.85E-4 0.00E+0 -9.07E-3 -7.59E-4
RWD [kg] 3.24E-3 4.21E-6 1.01E-4 0.00E+0 3.38E-4 2.35E-7 1.18E-4 6.27E-5 5.26E-5 -4.55E-5 0.00E+0 -1.45E-3 -5.27E-5
CRU [kg] 0.00E+0 0.00E+0 0.00E+0 0.00E+0 0.00E+0 0.00E+0 0.00E+0 0.00E+0 0.00E+0 0.00E+0 0.00E+0 0.00E+0 0.00E+0
MFR [kg] 7.64E-3 0.00E+0 9.20E-2 0.00E+0 0.00E+0 0.00E+0 0.00E+0 2.59E+0 0.00E+0 0.00E+0 0.00E+0 0.00E+0 0.00E+0
MER [kg] 0.00E+0 0.00E+0 0.00E+0 0.00E+0 0.00E+0 0.00E+0 0.00E+0 1.61E+0 0.00E+0 0.00E+0 0.00E+0 0.00E+0 0.00E+0
EEE [MJ] 0.00E+0 0.00E+0 2.43E-1 0.00E+0 0.00E+0 0.00E+0 7.87E+0 0.00E+0 0.00E+0 0.00E+0 0.00E+0 0.00E+0 0.00E+0
EET [MJ] 0.00E+0 0.00E+0 4.48E-1 0.00E+0 0.00E+0 0.00E+0 1.45E+1 0.00E+0 0.00E+0 0.00E+0 0.00E+0 0.00E+0 0.00E+0
HWD = Hazardous waste disposed; NHWD = Non-hazardous waste disposed; RWD = Radioactive waste disposed; CRU = Components
Caption for re-use; MFR = Materials for recycling; MER = Materials for energy recovery; EEE = Exported electrical energy; EEE = Exported
thermal energy
Not all of the life cycle inventories applied in this study support the methodological approach for the waste and
water indicators. The data are based on publications of industry. The indicators for waste and water of the system
are evaluated but contain a higher degree of uncertainty.
References
EN 1307
DIN EN 1307: 2014+A1:2016: Textile floor coverings - ecoinvent 3.6
Classification ecoinvent, Zurich, Switzerland, database version 3.6,
published September 2019
EN 13501-1
DIN EN 13501-1:2010-01: Fire classification of GaBi database 2020
construction products and building elements - Part 1: GaBi Software-System and Database for Life Cycle
Classification using data from reaction to fire tests Engineering, thinkstep AG, Leinfelden-Echterdingen,
service pack 40, 2020
EN 14041
DIN EN 14041: 2008-05: Resilient, textile and laminate IBU 2016
floor coverings - Essential characteristics IBU (2016): General Programme Instructions for the
Preparation of EPDs at the Institut Bauen und Umwelt
EN 15804 e.V., Version 1.1 Institut Bauen und Umwelt e.V.,
EN 15804:2012-04+A1 2013/, Sustainability of Berlin.
construction works — Environmental Product www.ibu-epd.de
Declarations — Core rules for the product category of
construction products PCR Part A
Product Category Rules for Construction Products
EN 16810 from the range of Environmental Product Declarations.
DIN EN 16810: 2017-08: Resilient, textile and laminate Part A: Calculation Rules for the Life Cycle
floor coverings – Environmental product declarations – Assessment and Requirements on the Background
Product category rules Report, V1.8, Berlin: Institut Bauen und Umwelt e.V.
(IBU), July 2019
ISO 10874
DIN EN ISO 10874: 2012-04: Resilient, textile and PCR Part B
laminate floor coverings - Classification Product Category Rules for Construction Products
from the range of Environmental Product Declarations
ISO 14025 of Institut Bauen und Umwelt (IBU),
DIN EN /ISO 14025:2011-10/, Environmental labels Part B: Requirements on the EPD for floor coverings,
and declarations — Type III environmental V1.2, Berlin: Institut Bauen und Umwelt e.V. (IBU),
declarations — Principles and procedures February 2018
ISO 15686 PRODIS
ISO 15686: Buildings and constructed assets - Product Information System (PRODIS) of the
Service life planning European Carpet Industry, Gemeinschaft
ISO 15686-1: 2011-05: Part 1: General principles and umweltfreundlicher Teppichboden e.V (GUT) and
framework European Carpet and Rug Association
ISO 15686-2: 2012-05: Part 2: Service life prediction (ECRA), http://www.pro-dis.info
procedures
ISO 15686-7: 2006-03: Part 7: Performance REACH
evaluation for feedback of service life data Regulation (EC) No 1907/2006 of the European
from practice Parliament and of the Council of 18 December 2006
ISO 15686-8: 2008-06: Part 8: Reference service life concerning the Registration, Evaluation, Authorisation
and service-life estimation and Restriction of Chemicals (REACH). Last update:
25.03.2014 (Status: 27.06.2018)
Regulation (EU) No. 305/2011
Regulation No. 305/2011 Construction Products VDZ e.V.
Regulation (CPR) of the European Council and of the Association of German Cement Works, Ed.
European Parliament, April 2011 Environmental Data of the German Cement Industry
2018
CML
Institute of Environmental Sciences - in Dutch
'Centrum voor Milieuwetenschappen in Leiden' (CML),
Leiden, The Netherlands
6 Environmental Product Declaration Balsan – PILOTE² - tufted carpet tiles
Publisher
Institut Bauen und Umwelt e.V. Tel +49 (0)30 3087748- 0
Panoramastr. 1 Fax +49 (0)30 3087748- 29
10178 Berlin Mail info@ibu-epd.com
Germany Web www.ibu-epd.com
Programme holder
Institut Bauen und Umwelt e.V. Tel +49 (0)30 - 3087748- 0
Panoramastr 1 Fax +49 (0)30 – 3087748 - 29
10178 Berlin Mail info@ibu-epd.com
Germany Web www.ibu-epd.com
Author of the Life Cycle
Assessment Tel +49 (0)241 96843 410
Gemeinschaft umweltfreundlicher Fax +49 (0)241 96843 400
Teppichboden (GUT) e.V. Mail mail@gut-ev.de
Schönebergstraße 2 Web www.gut-ev.org
52068 Aachen
Germany
Owner of the Declaration
Balsan Moquette Tel +33 (0) 254 2916 00
Corbilly 2 Fax +33 (0) 254 3679 08
36330 Arthon Mail cedric.charton@balsan.com
France Web www.balsan.com
