ENVIRONMENTAL PRODUCT DECLARATION
as per ISO 14025 and EN 15804+A2
Owner of the Declaration Knauf Integral KG
Publisher Institut Bauen und Umwelt e.V. (IBU)
Programme holder Institut Bauen und Umwelt e.V. (IBU)
Declaration number EPD-KNA-20220092-CAB1-EN
Issue date 26.06.2023
Valid to 25.06.2028
Knauf GIFAfloor DB 30 green
Knauf Integral KG
www.ibu-epd.com | https://epd-online.com
General Information
Knauf Integral KG Knauf GIFAfloor DB 30 green
Programme holder Owner of the declaration
IBU – Institut Bauen und Umwelt e.V. Knauf Integral KG
Hegelplatz 1 Am Bahnhof 16
10117 Berlin 74589 Satteldorf
Germany Germany
Declaration number Declared product / declared unit
EPD-KNA-20220092-CAB1-EN 1 m² of gypsum fibre panel Knauf GIFAfloor DB 30 green, 48.3 kg/m², 30
mm
This declaration is based on the product category rules: Scope:
Plasterboard, 01.08.2021 This EPD declares the environmental impacts of the gypsum fibre panels
(PCR checked and approved by the SVR) Knauf GIFAfloor DB 30 green, produced by Knauf Integral KG, plant
Satteldorf (Germany). It covers 100 % of the manufacture of Knauf
GIFAfloor DB 30 green in Satteldorf (D). The life cycle assessment is
Issue date based on production data for 2020.
The owner of the declaration shall be liable for the underlying information
26.06.2023
and evidence; the IBU shall not be liable with respect to manufacturer
information, life cycle assessment data and evidences.
Valid to
The EPD was created according to the specifications of EN 15804+A2. In
25.06.2028 the following, the standard will be simplified as EN 15804.
Verification
The standard EN 15804 serves as the core PCR
Independent verification of the declaration and data according to ISO
14025:2011
internally X externally
Dipl.-Ing. Hans Peters
(Chairman of Institut Bauen und Umwelt e.V.)
Dipl.-Ing. Hans Peters Dr Naeem Adibi,
(Managing Director Institut Bauen und Umwelt e.V.) (Independent verifier)
1 Environmental Product Declaration - Knauf Integral KG - Knauf GIFAfloor DB 30 green
Product
Product description/Product definition This product contains other CMR substances in categories 1A
The declared product Knauf GIFAfloor DB 30 green is a or 1B (Regulation (EC) No. 1272/2008) which are not on the
gypsum fibre board made of gypsum with paper fibres candidate list, exceeding 0.1 percentage by mass: no
suspended in the gypsum matrix for reinforcement of the
boards. The declared products have a thickness of 30 mm. Biocide products were added to this construction product or it
Further thicknesses (36 mm, 40 mm) are declared in separate has been treated with biocide products (this then concerns a
EPDs. treated product as defined by the (EU) Ordinance on Biocide
For the placing on the market of the product in the European Products No. 528/2012): no
Union/European Free Trade Association (EU/EFTA) (with the
exception of Switzerland) Regulation (EU) No. 305/2011 (CPR) Reference service life
applies. The product needs a declaration of performance No reference service life according to ISO 15686 has been
taking into consideration EN 15283-2:2008 + A1:2009, Gypsum determined for the declared products. However, a service life of
boards with fibrous reinforcement - Definitions, ≥ 50 years can be assumed for raised access floor panels
requirements and test methods - Part 2: Gypsum fibre boards according to the BBSR table "Service lives of components for
and the CE-marking. life cycle assessment according to BNB" (code no. 352.911).
There are no influences on ageing when the panels are applied
National provisions apply for the application and use. in accordance with the rules of technology.
Application Extraordinary effects
Knauf GIFAfloor DB green boards are used as raised access
floors panels with loose laid carpets or for access openings in Fire protection
dry hollow floor systems. Building material class A1
Burning droplets -
Applicable standards are: Smoke gas development -
• EN 12825:2001, Raised access floors
• EN 13213:2001, Hollow floors Contact with water
Knauf GIFAfloor DB 30 green are designed to tolerate relative
Technical Data humidities up to 75 %. Exceeding humidities or permanent
Technical datasheets can be downloaded from the website exposure to wet conditions may lead to a decrease in strength
https://www.knauf-integral.de. and should be avoided. However, due to the ingredients no
negative effect on human health is to be expected from
Constructional data of Knauf GIFAfloor DB 30 green
leaching.
Name Value Unit
Gross density acc. to EN 15283-2 ≥ 1500 kg/m3 An instruction sheet about the restoration of flood damage is
Thermal conductivity acc. to EN ISO 10456 0.25 W/mK available under www.knauf.de /BSDH/. Information about the
removal of flood damage can also be downloaded from
Calculation value for thermal conductivity 0.44 W/mK
www.gypsum.org.
Specific heat capacity 1 kJ/kgK
Due to the loose laying of Knauf GIFAfloor DB green panels
Water vapour diffusion resistance factor acc. to 10 - affected panels can be easily replaced by new ones.
EN ISO 10456
Water vapour diffusion resistance factor acc. to Re-use
4 -
EN ISO 10456 Knauf GIFAfloor DB 30 green panels are laid loosely on the
0.5 - sub-construction and is typically covered by self-laid loose
Moisture content at 20 °C, 65% humidity M.-%
0.9 textile covering. Therefore, they can be removed without any
damage to the panels and re-use is possible.
Elongation/Vibration when humidity changes by
≤ 1.00 mm/m
30% (20°C) acc. to EN 318
According to the German Commercial Waste Ordinance
Performance data of the product in accordance with the GewAbfV construction and demolition based on gypsum is
declaration of performance with respect to its essential preferably collected separately from other waste types and
characteristics according to EN 15283-2:2008 + A1:2009, supplied to recycling facilities. In addition, Knauf GIFAfloor DB
Gypsum boards with fibrous reinforcement - Definitions, 30 green panels are designed to be easily recyclable.
requirements, and test methods - Part 2: Gypsum fibre boards.
Disposal
Base materials/Ancillary materials
Knauf GIFAfloor DB 30 green panels need to be dismanteled
Knauf GIFAfloor DB green panels consist of approx. 92 % w/w
and collected separately from other construction waste. If
set gypsum reinforced with > 7 % w/w paper fibres and < 0.5 %
disposed, Knauf GIFAfloor DB 30 green panels need to be
additives. Knauf GIFAfloor DB green panels are impregnated
disposed of as gypsum waste under the European Waste Code
with < 0.5 % w/w impregnating agent (surface impregnation).
(EWC)
The declared products contains substances listed in the
17 08 02 - gypsum-based construction materials other than
candidate list (date: 17.01.2023, ECHA2022) exceeding 0.1
those mentioned in 17 08 01
percentage by mass: no.
LCA: Calculation rules
2 Environmental Product Declaration - Knauf Integral KG - Knauf GIFAfloor DB 30 green
way, gypsum becomes settled and hardened. Redundant
Declared Unit surface water is finally removed in a dryer.
The declared unit is 1 m² of Knauf GIFAfloor DB 30 green
panels. The conversion factors and densities are given in the
table below: Cut-offs
Declared unit for Knauf GIFAfloor DB 30 green Cut-off rules as required by EN 15804+A2 are respected. The
details are given in the background report. The environmental
Name Value Unit
impacts imposed by these cut-offs are considered neglectable.
Declared unit 1 m2 In total, the cut off materials and processes are less than 5 % of
conversion factor [Mass/Declared Unit] to 1 kg 0.021 - the mass and energy flows in the modules (A1-A3).
Grammage 48.3 kg/m2
Gross density ≥ 1500 kg/m3
Data quality
Layer thickness 0.03 m Datasets exclusively from GaBi databases (version 2022.1) are
The declared environmental impacts are average impacts for used for the LCA modelling. All datasets used have been
the production in plant Satteldorf. Water and energy updated in the last 5 years. For processes and materials, where
consumption is measured on an annual basis and allocated to no direct match is available, data from literature or expert
the various products by the annually produced surface area per judgements are applied. Only a few materials and processes
panel thickness. needed to be cut off due to missing information. Since these
cut-off materials and processes are only of small amounts (<< 1
Knauf Integral plant Satteldorf is specifically designed to % w/w), the total influence of these neglected inputs is
produce a fibre reinforced gypsum material called Knauf expected to be lower than 5 % of energy usage and mass.
GIFAtec which is adapted in shape, density, surface treatment,
and edge trimming to yield the desired products. Therefore, With respect to technological, geographic and time
results of the life cycle indicators are considered to be very representativeness, the overall data quality
robust. is evaluated to be 'satisfactory'.
The LCA was modeled with software GaBi and its Foreground data are related to production data from plant
corresponding databases (database version 2022.1). Satteldorf for the reference year 2020. Water and energy
consumption are monitored and reported on an annual basis
and allocated to the specific products based on annually
System boundary produced surface area per panel thickness. Since the
Type of the EPD: cradle to gate - with options, modules C1–C4, composition of the material is quite constant throughout the
and module D (A1–A3 + C+ D, additional modules: A4, A5) product range, the LCA results are considered to be quite
This EPD includes the following life cycle stages: robust with respect to the foreground data.
• provision of raw materials and transport to plant
Allocations
Satteldorf, production of boards (A1-A3) including
Allocations in the foreground data have only been applied for
thermal energy for calcination and drying (from natural
energy and water consumption data which is monitored on an
gas, geographic scope: DE), as well as electricity
annual basis for the whole production plant Satteldorf.
(residual mix DE) transport to building site (A4)
Allocations in the background data are described and have not
• installation at building site (A5) including the incineration
been adjusted. Paper fibres incorporated in the gypsum fibre
of transport packaging,
panels are made from waste cardboard and enter the product
• manual disassembly (C1)
system free of burdens. Further allocations of production data
• transport to recycling facility or landfill site (C2)
have been avoided.
• 2 scenarios for end of life:
• Scenario 1: landfilling (C4/1), corresponding to zero
However, there may be allocations in the background data
impacts in C3/1 and credits in D/1 from incineration of
which are are explained in the documentation of the respective
packaging material in A5
datasets.
• Scenario2: recycling (C3/2), zero impacts in C4/2 and
credits for the recycled material beyond the system
Geographic Representativeness
boundaries and from A5 (D/2). Recycling includes the
Land or region, in which the declared product system is
electrical energy for the crushing and grinding of the
manufactured, used or handled at the end of the product´s
disassembled panels prior to backfeeding into the next
lifespan: Global
production cycle.
Fig. 1 illustrates the production process: Natural and Flue gas Comparability
desulphurization (FGD) gypsum is calcined (removal of water of
Basically, a comparison or an evaluation of EPD data is only
crystallization). The calcined stucco in mixed with additive and
possible if all the data sets to be compared were created
fibres from wastepaper and mixed with water. This slurry is fed
according to EN 15804 and the building context, respectively
to an infinite belt with vacuum pumps. After this, the density of
the product-specific characteristics of performance, are taken
the material is adjusted by a winding roller and a press. Mixing
into account.
with water leads to the re-incorporation of water of
crystallization into the crystal lattice of calcium sulphate. That
3 Environmental Product Declaration - Knauf Integral KG - Knauf GIFAfloor DB 30 green
Fig. 1: Production process for gypsum fibre panels
LCA: Scenarios and additional technical information
freight ship are required for transportation. Due to these
Characteristic product properties of biogenic carbon different transportation vehicles employed, the transport
Information on describing the biogenic Carbon Content at distances for FGD gypsum were calculated with weighted
factory gate averages for a combined transportation by truck, river, and
ocean.
Name ValueUnit
kg
Biogenic carbon content in product 1.89 Further raw materials are supplied by truck from manufacturers
C
within Germany or from neighboring countries.
Biogenic carbon content in accompanying kg
0.082
packaging C Manufacturing
Gypsum (natural and FGD gypsum) is calcined to stucco before
mixing with water. Stucco, cellulose fibres and small amounts of
Product Stage (A1-A3)
additives are then suspended in water to give a slurry. The
resulting mixture passes a job feeder and is fed on an infinite
Supply of raw materials
felt with vacuum pumps to remove excess water. Afterwards,
Knauf GIFAfloor DB green boards are gypsum fibre boards
the pulp is driven through a winding roller and a subsequent
consisting of gypsum with cellulose fibre from recycled
press for panel forming and further removal of water before it
cardboard incorporated in the gypsum matrix. Currently, natural
finally enters a dryer. Drying of surface moisture is followed by
gypsum from open-cast mining in close vicinity to the
surface finishing, formatting and edge processing as well as the
production plant as well as gypsum from the flue gas
application of the impregnating agent.
desulphurization of different coal-fired power plants is used to
produce the boards.
(Transport) Packaging
Knauf GIFAfloor DB green panels are not packaged individually,
Small amounts of additives are used for easier processing and
but stacked on a wooden pallet (reusable), covered with a
fine adjustment of properties.
cardboard sheet and secured with PET straps.
Transport of raw materials
Natural gypsum is extracted from mines close to the Transport to the building site (A4)
manufacturing sites. Accordingly, transport distances are short As the default value, transportation over 500 km by truck was
(< 30 km) and trucks are used. FGD gypsum is transported by assumed for the transportation of the products to the building
truck from coal-fired power plants in Germany and Europe, site. This is no actual transport distances since transport
mainly. In few cases, a river freight ship and even an ocean distance can only be considered at the building level.
4 Environmental Product Declaration - Knauf Integral KG - Knauf GIFAfloor DB 30 green
Nevertheless, the provided numbers shall enable the A service life of ≥ 50 years can be assumed for raised access
calculation of the actual environmental burdens for the floor panels and ceiling and wall coverings according to the
transport of the declared products by inter-/extrapolating BBSR table "Service lives of components for life cycle
distances and mixing of transport means according to assessment according to BNB".
the conditions at hand for individual building assessments.
Hygrothermal in-use conditions (stationary): -10 °C to +35 °C;
However, since Knauf GIFAfloor DB green panels are shipped 35 to 75 % rel. air humidity
globally, further transportation scenarios were considered:
End of life (C1-C4)
- Scenario (A4/1): Transport by truck 1000 km
Knauf GIFAfloor DB 30 green are disassembled manually and
- Scenario (A4/2): Transport by rail 1000 km
collected separately from other deconstruction waste.
- Scenario (A4/3): Transport by ocean freight ship over 10 000
Transportation in C2 is assumed to be 100 km by truck to either
km
an appropriate landfill site (scenario 1) or to a recycling facility
- Scenario (A4/4): Transport by river freight ship over 1000 km
(scenario 2).
The results of these further transportation scenarios are given
in the Annexe to this EPD.
Since Knauf GIFAfloor DB 30 green are laid loosely, no
adhering foreign material needs to be removed from the panels
Default scenario (A4): Transport by truck 500 km
prior to recycling (scenario 2). The panels are milled to fine
Name Value Unit powder without any further material separation. The same
Litres of fuel 0.113 l/100km energy consumption as for the milling of natural gypsum in
Transport distance 500 km plant Satteldorf is assumed for the recycling procedure. The
recycled gypsum is assumed to replace virgin FGD and natural
Capacity utilisation (including empty runs) 50 %
gypsum in the same ratio as it was initially introduced into
Gross density of products transported ≥ 1500 kg/m3
production cycle declared in modules A1-A3. No additional
processes are required for recycling.
Installation into the building (A5)
Raised access floor panels Knauf GIFAfloor DB green are
installed by being loosely laid on specific raised access floor
Name ValueUnit
pedestals available at Knauf Integral KG according to
the installation instructions. No sealing of joints is required. Collected separately gypsum-based construction
48.3 kg
materials
Name Value Unit
Landfilling scenario 1 48.3 kg
Electricity consumption - kWh
Recycling scenario 2 48.3 kg
Type of assembly manually
Construction waste 5 % With the definition of 2 end-of-life scenarios, benefits and loads
beyond system boundaries are declared as follows:
Treatment of packaging
incineration D/1: contains only credits for exported energy from incineration
waste
of packaging material (results only from A5)
Components not Substructures, screws, jointing
D/2: contains credits for exported energy from incineration of
considered material
packaging material in A5 and the benefits from the recycled
material of Knauf GIFAfloor DB green panels replacing FGD
Use phase (B1-B7): Excluded since no environmental and natural gypsum in the same ratio as both gypsum types
impacts/benefits are expected. were introduced in A1-A3; amount of paper fibres is discounted
from weight of demolition waste to avoid double counting of
secondary material and replacement of gypsum by paper fibres.
5 Environmental Product Declaration - Knauf Integral KG - Knauf GIFAfloor DB 30 green
LCA: Results
Note: Two scenarios for the end of life stage were considered as 100 % scenario, each.
Scenario 1: 100 % Landfilling - module C4/1, C3/1 with zero impacts, D/1 (only from A5)
Scenario 2: 100 % Recycling - modules C3/2, C4/2 with zero impacts, D/2 (from A5 and C3/2)
DESCRIPTION OF THE SYSTEM BOUNDARY (X = INCLUDED IN LCA; ND = MODULE OR INDICATOR NOT DECLARED; MNR =
MODULE NOT RELEVANT)
Benefits and
Construction loads beyond
Product stage Use stage End-of-life stage
process stage the system
boundaries
la ire ta m w a Ry lp p u s tro p s n a rT g n iru tc a fu n a M e h t m o rf tro p s n a rTe tis e h t o t e ta g y lb m e s s A e s U e c n a n e tn ia M ria p e R tn e m e c a lp e R tn e m h s ib ru fe R y g re n e la n o ita re p Oe s u re ta w la n o ita re p Oe s u n o itc u rts n o c -e Dn o itilo m e d tro p s n a rT g n is s e c o rp e ts a W la s o p s iD -e s u e R-y re v o c e R-g n ilc y c e Rla itn e to p
A1 A2 A3 A4 A5 B1 B2 B3 B4 B5 B6 B7 C1 C2 C3 C4 D
X X X X X MND MND MNR MNR MNR MND MND X X X X X
RESULTS OF THE LCA - ENVIRONMENTAL IMPACT according to EN 15804+A2: 1 m² Knauf GIFAfloor DB 30 green, 48.3 kg/m²,
30 mm
Parameter Unit A1-A3 A4 A5 C1 C2 C3/1 C3/2 C4/1 C4/2 D/1 D/2
GWP-total kg CO 2 eq 1.76E+00 1.7E+00 1.19E+00 0 3.44E-01 0 6.96E+00 7.85E+00 0 -1.08E-01 -7.18E+00
GWP-fossil kg CO 2 eq 8.96E+00 1.7E+00 6.12E-01 0 3.42E-01 0 4.98E-02 9.38E-01 0 -1.08E-01 -2.6E-01
GWP-
biogenic kg CO 2 eq -7.21E+00 0 5.79E-01 0 0 0 6.91E+00 6.91E+00 0 -5.51E-04 -6.92E+00
GWP-luluc kg CO 2 eq 1.71E-03 6.47E-03 5.92E-04 0 2.29E-03 0 1.05E-05 1.36E-03 0 -1.18E-05 -1.38E-04
kg CFC11
ODP 2.06E-11 3.88E-13 1.18E-12 0 4.2E-14 0 7.28E-13 1.93E-12 0 -7.28E-13 -1.21E-12
eq
AP mol H+ eq 2.78E-02 1.65E-03 1.84E-03 0 3.85E-04 0 1.09E-04 6.03E-03 0 -1.42E-04 -5.21E-04
EP-
kg P eq 2.7E-06 3.36E-06 1.89E-06 0 1.22E-06 0 1.45E-07 3.04E-05 0 -1.48E-07 -3.13E-07
freshwater
EP-marine kg N eq 8.1E-03 5.75E-04 5.56E-04 0 1.28E-04 0 2.45E-05 1.98E-03 0 -3.84E-05 -1.89E-04
EP-terrestrial mol N eq 9.01E-02 6.57E-03 6.04E-03 0 1.49E-03 0 2.57E-04 1.8E-02 0 -4.12E-04 -2.13E-03
kg NMVOC
POCP 2.25E-02 1.48E-03 1.59E-03 0 3.32E-04 0 6.62E-05 6.45E-03 0 -1.08E-04 -5.03E-04
eq
ADPE kg Sb eq 2.59E-06 1.7E-07 1.45E-07 0 3.46E-08 0 1.36E-08 8.67E-08 0 -1.63E-08 -3.01E-08
ADPF MJ 1.29E+02 2.25E+01 8.49E+00 0 4.51E+00 0 9.03E-01 1.24E+01 0 -1.83E+00 -3.52E+00
m3 world eq
WDP 4.79E-01 8.01E-03 6.4E-02 0 3.96E-03 0 1.13E-02 9.18E-02 0 -1.15E-02 -1.32E-02
deprived
GWP = Global warming potential; ODP = Depletion potential of the stratospheric ozone layer; AP = Acidification potential of land and water; EP =
Eutrophication potential; POCP = Formation potential of tropospheric ozone photochemical oxidants; ADPE = Abiotic depletion potential for non-fossil
resources; ADPF = Abiotic depletion potential for fossil resources; WDP = Water (user) deprivation potential)
RESULTS OF THE LCA - INDICATORS TO DESCRIBE RESOURCE USE according to EN 15804+A2: 1 m² Knauf GIFAfloor DB
30 green, 48.3 kg/m², 30 mm
Parameter Unit A1-A3 A4 A5 C1 C2 C3/1 C3/2 C4/1 C4/2 D/1 D/2
PERE MJ 4.09E+00 1.49E+00 6.61E+00 0 3.13E-01 0 6.39E+01 1.62E+00 0 -5.03E-01 -6.41E+01
PERM MJ 6.63E+01 0 -2.9E+00 0 0 0 -6.34E+01 0 0 0 6.34E+01
PERT MJ 7.03E+01 1.49E+00 3.71E+00 0 3.13E-01 0 5.01E-01 1.62E+00 0 -5.03E-01 -7.5E-01
PENRE MJ 1.29E+02 2.25E+01 8.58E+00 0 4.52E+00 0 9.03E-01 1.24E+01 0 -1.83E+00 -3.52E+00
PENRM MJ 8.85E-02 0 -8.85E-02 0 0 0 0 0 0 0 0
PENRT MJ 1.29E+02 2.25E+01 8.5E+00 0 4.52E+00 0 9.03E-01 1.24E+01 0 -1.83E+00 -3.52E+00
SM kg 3.68E+00 0 0 0 0 0 0 0 0 0 -4.46E+01
RSF MJ 0 0 0 0 0 0 0 0 0 0 0
NRSF MJ 0 0 0 0 0 0 0 0 0 0 0
FW m3 2.28E-02 1.18E-03 2.18E-03 0 3.66E-04 0 4.78E-04 2.76E-03 0 -4.84E-04 -7.78E-04
PERE = Use of renewable primary energy excluding renewable primary energy resources used as raw materials; PERM = Use of renewable primary
energy resources used as raw materials; PERT = Total use of renewable primary energy resources; PENRE = Use of non-renewable primary energy
excluding non-renewable primary energy resources used as raw materials; PENRM = Use of non-renewable primary energy resources used as raw
materials; PENRT = Total use of non-renewable primary energy resources; SM = Use of secondary material; RSF = Use of renewable secondary fuels;
NRSF = Use of non-renewable secondary fuels; FW = Use of net fresh water
RESULTS OF THE LCA – WASTE CATEGORIES AND OUTPUT FLOWS according to EN 15804+A2:
1 m² Knauf GIFAfloor DB 30 green, 48.3 kg/m², 30 mm
Parameter Unit A1-A3 A4 A5 C1 C2 C3/1 C3/2 C4/1 C4/2 D/1 D/2
HWD kg 2.18E-08 1.44E-10 1.15E-09 0 3.3E-11 0 7.81E-11 1.02E-09 0 -2.48E-10 -2.87E-10
NHWD kg 7.57E-02 3.71E-03 2.37E+00 0 7.46E-04 0 6.8E-04 4.74E+01 0 -9.26E-04 -1.6E-03
6 Environmental Product Declaration - Knauf Integral KG - Knauf GIFAfloor DB 30 green
RWD kg 5.77E-03 3.03E-05 3.02E-04 0 8.77E-06 0 1.44E-04 1.41E-04 0 -1.44E-04 -1.7E-04
CRU kg 0 0 0 0 0 0 0 0 0 0 0
MFR kg 0 0 0 0 0 0 4.83E+01 0 0 0 0
MER kg 0 0 1.86E-01 0 0 0 0 0 0 0 0
EEE MJ 0 0 4.84E-01 0 0 0 0 0 0 0 0
EET MJ 0 0 8.71E-01 0 0 0 0 0 0 0 0
HWD = Hazardous waste disposed; NHWD = Non-hazardous waste disposed; RWD = Radioactive waste disposed; CRU = Components for re-use;
MFR = Materials for recycling; MER = Materials for energy recovery; EEE = Exported electrical energy; EET = Exported thermal energy
RESULTS OF THE LCA – additional impact categories according to EN 15804+A2-optional:
1 m² Knauf GIFAfloor DB 30 green, 48.3 kg/m², 30 mm
Parameter Unit A1-A3 A4 A5 C1 C2 C3/1 C3/2 C4/1 C4/2 D/1 D/2
Disease
PM 8.06E-07 1.05E-08 4.47E-08 0 2.64E-09 0 9.05E-10 7.06E-08 0 -1.17E-09 -3.47E-07
incidence
IR kBq U235 eq 4.56E-01 3.08E-03 2.46E-02 0 1.3E-03 0 2.44E-02 1.71E-02 0 -2.44E-02 -2.71E-02
ETP-fw CTUe 4.77E+01 1.71E+01 3.85E+00 0 3.18E+00 0 3.95E-01 8.42E+00 0 -4.02E-01 -1.02E+00
HTP-c CTUh 1.44E-09 3.44E-10 1.4E-10 0 6.55E-11 0 1.14E-11 9.04E-10 0 -1.85E-11 -3.34E-11
HTP-nc CTUh 1.22E-07 1.73E-08 1.23E-08 0 3.55E-09 0 4.15E-10 1.02E-07 0 -7.1E-10 -1.62E-09
SQP SQP 4.93E+01 6.7E+00 3.02E+00 0 1.89E+00 0 3.26E-01 2.16E+00 0 -3.27E-01 -8.63E-01
PM = Potential incidence of disease due to PM emissions; IR = Potential Human exposure efficiency relative to U235; ETP-fw = Potential comparative
Toxic Unit for ecosystems; HTP-c = Potential comparative Toxic Unit for humans (cancerogenic); HTP-nc = Potential comparative Toxic Unit for humans
(not cancerogenic); SQP = Potential soil quality index
Disclaimer 1 – for the indicator “Potential Human exposure efficiency relative to U235”. This impact category deals mainly with the
eventual impact of low dose ionizing radiation on human health of the nuclear fuel cycle. It does not consider effects due to possible
nuclear accidents, occupational exposure nor due to radioactive waste disposal in underground facilities. Potential ionizing radiation
from the soil, from radon and from some construction materials is also not measured by this indicator.
Disclaimer 2 – for the indicators “abiotic depletion potential for non-fossil resources”, “abiotic depletion potential for fossil resources”,
“water (user) deprivation potential, deprivation-weighted water consumption”, “potential comparative toxic unit for ecosystems”,
“potential comparative toxic unit for humans – cancerogenic”, “Potential comparative toxic unit for humans - not cancerogenic”,
“potential soil quality index”. The results of this environmental impact indicator shall be used with care as the uncertainties on these
results are high or as there is limited experienced with the indicator.
References
Standards declarations — Type III environmental declarations —
EN 318 Principles and procedures.
EN 318:2002-06 Wood-based panels - Determination of
dimensional changes associated with changes in relative ISO 14040
humidity ISO 14040:2006 + Amd 1:2020, Environmental management –
Life cycle assessment – Principles and framework
EN ISO 10456
EN ISO 10456:2010-05, Building materials and products - ISO 14044
Hygrothermal properties - Tabulated design values and ISO 14044:2006 + Amd 1:2017 + Amd 2:2020, Environmental
procedures for determining declared and design thermal values management – Life cycle assessment – Requirements and
(ISO 10456:2007 + Cor. 1:2009) guidelines
EN 12825 ISO 15686
EN 12825:2001, Raised access floors ISO 15686-2:2012-05, Buildings and constructed assets -
Service life planning - Part 2: Service life prediction
EN 13213 procedures
EN 13213:2001, Hollow floors
Further References
EN 13501 BBSR
EN 13501-1: 2018, Fire classification of construction products table "Service lives of components for life cycle assessment
and building elements - Part 1: Classification using data from according to BNB" http://www.nachhaltigesbauen.de/baustoff-
reaction to fire tests und-gebaeudedaten/nutzungsdauern-von-bauteilen.html,
published 2017, last accessed 2022-09-29
EN 15283
EN 15283-2:2008 + A1:2009, Gypsum boards with fibrous ECHA
reinforcement - Definitions, requirements, and test methods - European Chemicals Agency (ECHA), Candidate List of
Part 2: Gypsum fibre boards Substances of Very High Concern for Authorisation (published
in
EN 15804 accordance with Article 59(10) of the REACH Regulation),
EN 15804:2019+A2, Sustainability of construction works — http://echa.europa.eu/de/candidate-list-table, Revision: 2023-
Environmental Product Declarations — Core rules for the 01-17
product category of construction products.
European Waste Code
ISO 14025 Guidance on classification of waste according to EWC-Stat
DIN EN ISO 14025:2011-10, Environmental labels and categories, Supplement to the Manual for the Implementation of
7 Environmental Product Declaration - Knauf Integral KG - Knauf GIFAfloor DB 30 green
the Regulation (EC) No 2150/2002 on Waste Statistics, Project Report according to EN 15804+A2:2019, v1.1.2, 2021-
COMMISSION OF THE EUROPEAN 09-02
COMMUNITIES/EUROSTAT, v2, December 2010
IBU PCR Part B "Plasterboards"
GaBi Institut Bauen und Umwelt e.V.: PCR Guidance-Texts for
GaBi ts (v10.6.1.35): Software-System and Databases for Life Building-Related Products and Services Part B: Requirements
Cycle Engineering, Sphera Solutions GmbH, Leinfelden- on the EPD for Plasterboard, v1.7, 2019-01-04
Echterdingen, Germany, 2022 (database version 2022.1)
(EU) Ordinance on Biocide Products No. 528/2012
GewAbfV REGULATION (EU) No 528/2012 OF THE EUROPEAN
Verordnung über die Bewirtschaftung von gewerblichen PARLIAMENT AND OF THE COUNCIL of 22 May 2012
Siedlungsabfällen und von bestimmten Bau- und concerning the making available on the market and use of
Abbruchabfällen (Gewerbeabfallverordnung - biocidal products
GewAbfV) Gewerbeabfallverordnung vom 18. April 2017 (BGBl.
I S. 896), last amended by Artikel 3 der Verordnung vom Regulation (EU) No. 305/2011
28. April 2022 (BGBl. I S. 700) REGULATION (EU) No 305/2011 OF THE EUROPEAN
German Commercial Waste Ordinance PARLIAMENT AND OF THE COUNCIL of 9 March 2011
laying down harmonised conditions for the marketing of
IBU 2021 construction products and repealing Council Directive
Institut Bauen und Umwelt e.V.: Allgemeine Anleitung für das 89/106/EEC
EPD-Programm des Institut Bauen und Umwelt e.V. (IBU).
Version 2.0, Berlin: Institut Bauen und Umwelt e.V., 2021. Regulation (EC) No. 1272/2008
www.ibu-epd.com REGULATION (EC) No 1272/2008 OF THE EUROPEAN
PARLIAMENT AND OF THE COUNCIL of 16 December 2008
IBU PCR Part A on classification, labelling and packaging of substances
Institut Bauen und Umwelt e.V.: Product Category Rules for and mixtures, amending and repealing Directives 67/548/EEC
Building-Related Products and Services Part A: Calculation and 1999/45/EC, and amending Regulation (EC) No 1907/2006
Rules for the Life Cycle Assessment and Requirements on the
8 Environmental Product Declaration - Knauf Integral KG - Knauf GIFAfloor DB 30 green
Publisher
Institut Bauen und Umwelt e.V. +49 (0)30 3087748- 0
Hegelplatz 1 info@ibu-epd.com
10117 Berlin www.ibu-epd.com
Germany
Programme holder
Institut Bauen und Umwelt e.V. +49 (0)30 3087748- 0
Hegelplatz 1 info@ibu-epd.com
10117 Berlin www.ibu-epd.com
Germany
Author of the Life Cycle Assessment
Knauf Gips KG 0049 9001 31-1000 *
Am Bahnhof 7 knauf-direkt@knauf.de
97346 Iphofen www.knauf.de
Germany
Owner of the Declaration
Knauf Integral KG +49 (7951) 497-0
Am Bahnhof 16 info@knauf-integral.de
74589 Satteldorf https://www.knauf-integral.de/de/
Germany
9 Environmental Product Declaration - Knauf Integral KG - Knauf GIFAfloor DB 30 green
