ENVIRONMENTAL PRODUCT DECLARATION
as per ISO 14025 and EN 15804+A1
Owner of the Declaration Associated Weavers Europe NV
Programme holder Institut Bauen und Umwelt e.V. (IBU)
Publisher Institut Bauen und Umwelt e.V. (IBU)
Declaration number EPD-AWE-20220156-CBA1-EN
Issue date 25.05.2022
Valid to 24.05.2027
Sedna Range
Tufted broadloom carpet with a total pile weight of 2878
g/m2 and a pile material of 100% regenerated polyamide 6
Associated Weavers Europe NV
www.ibu-epd.com | https://epd-online.com
Umwelt Produktdeklaration Name des Herstellers – Name des Produkts
General Information
Associated Weavers Europe NV Sedna Range
Tufted broadloom carpet
Total pile weight of 2878 g/m2 100%
regenerated PA6 yarn
Textile polyester backing with 100%
recycled material
Programme holder Owner of the declaration
IBU – Institut Bauen und Umwelt e.V. Associated Weavers Europe NV
Hegelplatz 1 Industriepark Klein Frankrijk
10117 Berlin Weverijstraat 1
Germany 9600 Ronse
Belgium
Declaration number Declared product / declared unit
EPD-AWE-20220156-CBA1-EN Sedna Range - 1 m² tufted broadloom carpet with a
surface pile of 100% regenerated PA 6 and a polyester
Eco FusionBac backing.
This declaration is based on the product Scope:
category rules: The manufacturer declaration applies to broadloom
Floor coverings, 02/2018 carpets with Eco FusioBac, a pile material of PA 6 with
(PCR checked and approved by the SVR) 100% recycled content and a total pile weight of 2878
g/m2. The products are produced in Ronse, Belgium.
Issue date The declaration is only valid in conjunction with a valid
GUT-PRODIS license of the product.
25.05.2022
Valid to The owner of the declaration shall be liable for the
underlying information and evidence; the IBU shall not
24.05.2027
be liable with respect to manufacturer information, life
cycle assessment data and evidences.
The EPD was created according to the specifications
of EN 15804+A1. In the following, the standard will be
simplified as EN 15804.
Verification
The standard EN 15804 serves as the core PCR
Independent verification of the declaration and data
according to ISO 14025:2011
Dipl. Ing. Hans Peters internally x externally
(chairman of Institut Bauen und Umwelt e.V.)
Dr. Alexander Röder Angela Schindler
(Managing Director Institut Bauen und Umwelt e.V.)) (Independent verifier)
Product
Product description/Product definition Regulation (CPR) applies. The product needs a
Tufted broadloom carpets having a surface pile of Declaration of Performance (DoP) taking into
100% regenerated polyamide 6 and an Eco FusionBac consideration EN 14041: 2018-05, Resilient, textile and
backing. The colour of the carpet is generated by laminate floor coverings - Essential characteristics, and
continuous dyeing. The total recycled content amounts the CE-marking. The DoP of the product can be found
to 82% with a total pile weight of 2878 g/m2. The on the manufacturer's technical information section.
declaration applies to a product with a total pile weight For the application and use of the product the
of 2878 g/m2. respective national provisions apply.
For the placing on the market of the product in the Application
European Union/European Free Trade Association According to the use class as defined in EN 1307 the
(EU/EFTA) (with the exception of Switzerland) products can be used in all professional areas. The
Regulation (EU) No. 305/2011 Construction Product
2 Environmental Product Declaration Associated Weavers Europe NV (AW) – Sedna Range - Tufted Broadloom carpet with
a pile weight of 2878 g/m2 and 100% recycled PA6 yarn
use class can be found on the technical data sheet of This product contains substances listed in the ECHA
the product. candidate list (16.01.2020) or other carcinogenic,
mutagenic or reprotoxic (CMR) substances in
Technical Data categories 1A or 1B which are not on the candidate list
exceeding 0.1 percentage by mass: no.
The products are registered in the GUT-PRODIS
Information System. The PRODIS system ensures the
Name Value Unit compliance with limitations of various chemicals and
Product Form broadloom carpets - Volatile Organic Compound (VOC)-emissions and a
Type of manufacture Tufted carpets - ban on the use of all substances that are listed as
Yarn type Polyamide 6 - 'Substances of Very High Concern' (SVHC) under
continuous dyed REACH.
Coloration
surface
Primary backing Polypropylene Reference service life
Secondary backing Polyester - A calculation of the reference service life according to
Total pile weight max. 2878 g/m² ISO 15686 is not possible.
The service life of textile floor coverings strongly
Total carpet weight max. 3630 g/m2
depends on the correct installation taking into account
the declared use classification and the adherence to
cleaning and maintenance instructions.
Performance data of the product in accordance with
A minimum service life of 10 years can be
the declaration of performance with respect to its
assumed, technical service life can be considerably
essential characteristics according to EN 14041: 2018-
longer.
05, Resilient, textile and laminate floor coverings -
Essential characteristics. Additional product properties
in accordance with EN 1307 can be found on the
Product Information System PRODIS using the
PRODIS registration number of the product (www.pro-
dis.info) or on the manufacturer's technical information
section (www.carpetyourlife.com).
Base materials/Ancillary materials
Name Value Unit
Polyamide 6 79,3 %
Polyester 2,7 %
SBR-latex 3,6 %
Polypropylene 2,7 %
Limestone 11,7 %
Additives 0,01 %
LCA: Calculation rules
Declared Unit transport of the material to the manufacturing site,
emissions, waste water treatment, packaging material
and waste processing up to the landfill disposal of
Name Value Unit residual waste (except radioactive waste). Benefits for
Declared unit 1 m2 generated electricity and steam due to the incineration
Conversion factor to 1 kg 3.63 - of production waste are aggregated.
The declared unit refers to 1 m2 produced textile floor Biogenic carbon that is stored in renewable material
covering. The output of module A5 'Assembly' is 1 m2 (packaging paper) is taken into account as well as the
installed textile floor covering. associated carbon dioxide uptake from the air from
which this biogenic carbon comes.
System boundary A4 Transport:
Transport of the packed textile floor covering
Type of EPD: Cradle-to-grave from factory gate to the place of installation.
System boundaries of modules A, B, C, D: A5 Installation:
Modules C3, C4 and D are indicated separately for Installation of the textile floor covering, processing of
three end-of-life scenarios: installation waste and packaging waste up to the
1 - landfill disposal landfill disposal of residual waste (except radioactive
2 - municipal waste incineration waste), the production of the amount of carpet that
3 - recovery in a cement plant occurs as installation waste including its transport to
the place of installation.
Generated electricity and steam due to the incineration
of waste are listed in the result table as exported
A1-A3 Production: energy.
Energy supply and production of the basic material, Biogenic carbon that is stored in renewable materials
processing of secondary material, auxiliary material,
3 Environmental Product Declaration Associated Weavers Europe NV (AW) – Sedna Range - Tufted Broadloom carpet with
a pile weight of 2878 g/m2 and 100% recycled PA6 yarn
in packaging paper is released as carbon dioxide C3-3: Collection of the carpet waste for recovery in the
emissions into the air at the end of life in module A5. cement industry, waste processing (granulating),
Preparation of the floor and auxiliary materials transport to the cement plant, emissions from the
(adhesives, fixing agents, PET connectors) are beyond incineration. The biogenic carbon that is stored in the
the system boundaries and not taken into account. renewable materials of the floor covering is released
into the air as carbon dioxide emissions.
B1 Use:
Indoor emissions during the use stage. After the first C4 Disposal
year, no product-related Volatile Organic Compound C4-1: Impact from landfill disposal,
(VOC) emissions are relevant due to known VOC C4-2: The carpet waste leaves the system in
decay curves of the product. module C3-2,
C4-3: The pre-processed carpet waste leaves the
B2 Maintenance: system in module C3-3.
Cleaning of the textile floor covering for a period of 1
year: D Recycling potential:
Vacuum cleaning – electricity supply Calculated benefits result from materials exclusive
Wet cleaning – electricity, water consumption, secondary materials (net materials).
production of the cleaning agent, waste water D-A5: Benefits for generated energy due
treatment. to incineration of packaging and installation waste
The declared values in this module have to be (incineration plant with R1 > 0.6),
multiplied by the assumed service life of the floor D-1: Benefits for generated energy due to landfill
covering in the building in question. disposal of carpet waste at the end-of-life,
D-2: Benefits for generated energy due to incineration
B3 - B7: of carpet waste at the end-of-life (incineration plant
The modules are not relevant and therefore not with R1 > 0.6),
declared. D-3: Benefits for saved fossil energy and saved
inorganic material due to recovery of the carpet in a
C1 De-construction: cement plant.
The floor covering is de-constructed manually and no
additional environmental impact is caused. Comparability
Basically, a comparison or an evaluation of EPD data
C2 Transport: is only possible if all the data sets to be compared
Transport of the carpet waste to a landfill, to the were created according to EN 15804 and the building
municipal waste incineration plant (MWI) or to the context, respectively the product-specific
waste collection facility for recycling. characteristics of performance, are taken into account.
C3 Waste processing: Background data are taken from the GaBi database
C3-1: Landfill disposal needs no waste processing. 2021. Remaining data gaps are covered by the
C3-2: Impact from waste incineration (plant with ecoinvent 3.7 database
R1>0.6), generated electricity and steam are listed in
the result table as exported energy.
LCA: Scenarios and additional technical information
The following information refer to the declared modules anticipated strain on the floor by customers, the case-
and are the basis for calculations or can be used for specific useful life can be established. Based on this
further calculations. useful life the effects of Module B2 need to be
calculated in order to obtain the overall environmental
Transport to the construction site (A4) impacts.
Name Value Unit Name Value Unit
Litres of fuel (truck, EURO 0-6 mix) 0.0085 l/100km Maintenance cycle (wet cleaning) 1.5 1/year
Transport distance 700 km Maintenance cycle (vacuum cleaning) 208 1/year
Capacity utilisation (including empty Water consumption (wet cleaning) 0.004 m3
55 %
runs) Cleaning agent (wet cleaning) 0.09 kg
Electricity consumption 0.314 kWh
Installation in the building (A5) Further information on cleaning and maintenance see
Name Value Unit www.carpetyourlife.com
Material loss 0.33 kg
Polyethylene packaging waste and installation waste End of Life (C1-C4)
are considered to be incinerated in a municipal waste Three different end-of-life scenarios are declared and
incineration plant. Cardboard is going to be recycled. the results are indicated separately in module C.
Preparation of the floor and auxiliaries (adhesives, Each scenario is calculated as a 100 % scenario.
fixing agents, PET connectors etc.) are not taken into
account. Scenario 1: 100 % landfill disposal
Scenario 2: 100 % municipal waste incineration (MWI)
Maintenance (B2) with R1>0.6
The values for cleaning refer to 1 m2 floor covering Scenario 3: 100 % recycling in the cement industry
used in commercial areas per year. Depending on the
application based on ISO 10874, the technical service If combinations of these scenarios have to be
life recommended by the manufacturer and the calculated this should be done according to the
4 Environmental Product Declaration Associated Weavers Europe NV (AW) – Sedna Range - Tufted Broadloom carpet with
a pile weight of 2878 g/m2 and 100% recycled PA6 yarn
following scheme:
EOL-impact = x % impact (Scenario 1)
+ y % impact (Scenario 2)
+ z % impact (Scenario 3)
with x % + y % + z % = 100%
Name Value Unit
Collected as mixed construction waste
3.63 kg
(scenario 1 and 2)
Collected separately (scenario 3) 3.63 kg
Landfilling (scenario 1) 3.63 kg
Energy recovery (scenario 2) 3.63 kg
Energy recovery (scenario 3) 3,204 kg
Recycling (scenario 3) 0.426 kg
Reuse, recovery and/or recycling potentials (D),
relevant scenario information
Recovery or recycling potentials due to the three end-
of-life scenarios (module C) are indicated separately.
Recycling in the cement industry (scenario 3)
VDZ e.V.
The organic material of the carpet is used as
secondary fuel in a cement kiln. It mainly substitutes
for lignite (65.5 %), hard coal (26.2 %) and petrol coke
(8.6 %).
The inorganic material is substantially integrated into
the cement clinker and substitutes for original material
input.
5 Environmental Product Declaration Associated Weavers Europe NV (AW) – Sedna Range - Tufted Broadloom carpet with
a pile weight of 2878 g/m2 and 100% recycled PA6 yarn
LCA: Results
The LCA results refer to a declared product with a total pile weight of 2878 g/m2. The declared result figures in
module B2 have to be multiplied by the assumed service life (in years) of the floor covering in the building under
consideration. Information on non-relevant modules: Modules B3 - B7 are not relevant during the service life of
the carpet. Modules C1, C3/1, C4/2 and C4/3 cause no additional impact (see chapter "LCA: Calculation rules" in
this document). All these modules are declared and marked as 'modules not relevant/declared'. Module C2
represents the transport for scenarios 1, 2 and 3. Column D represents module D/A5. The calculations are based
on the CML characterization factors (version August 2016).
DESCRIPTION OF THE SYSTEM BOUNDARY (X = INCLUDED IN LCA; MND = MODULE NOT DECLARED;
MNR = MODULE NOT RELEVANT)
BENEFITS AND
CONSTRUCTI LOADS
PRODUCT STAGE ON PROCESS USE STAGE END OF LIFE STAGE BEYOND THE
STAGE SYSTEM
BOUNDARIES
6 Environmental Product Declaration Associated Weavers Europe NV (AW) – Sedna Range - Tufted Broadloom carpet with
a pile weight of 2878 g/m2 and 100% recycled PA6 yarn
lairetam
waR
ylppus tropsnarT
gnirutcafunaM
eht
morf
tropsnarT
etis
eht
ot
etag
ylbmessA esU
ecnanetniaM
riapeR
tnemecalpeR tnemhsibrufeR
ygrene
lanoitarepO esu
retaw
lanoitarepO esu
noitcurtsnoc-eD
noitilomed tropsnarT
gnissecorp
etsaW
lasopsiD -esueR -yrevoceR -gnilcyceR laitnetop
A1 A2 A3 A4 A5 B1 B2 B3 B4 B5 B6 B7 C1 C2 C3 C4 D
X X X X X X X MNR MNR MNR MND MND MND X X X X
RESULTS OF THE LCA - ENVIRONMENTAL IMPACT according to EN 15804+A1: 1 m² floorcovering
Parameter Unit A1-A3 A4 A5 B1 B2 C2 C3/2 C3/3 C4/1 D D/1 D/2 D/3
GWP [kg CO2-Eq.] 7.10E+0 2.13E-1 1.37E+0 0.00E+0 1.71E-1 1.20E-2 7.48E+0 7.57E+0 2.47E-1 -2.35E-2 0.00E+0 -1.67E-1 -4.30E-2
-3.57E- -2.49E- -1.88E-
ODP [kg CFC11-Eq.] 3.36E-8 3.71E-17 3.02E-9 0.00E+0 2.37E-9 2.10E-181.86E-152.51E-158.37E-16 0.00E+0
16 15 16
AP [kg SO2-Eq.] 2.96E-2 8.79E-4 3.47E-3 0.00E+0 4.46E-4 4.98E-5 8.00E-3 8.16E-3 6.40E-4 -2.71E-5 0.00E+0 -1.91E-4 -1.17E-4
EP [kg (PO4)3--Eq.] 6.62E-3 2.24E-4 8.06E-4 0.00E+0 9.11E-5 1.27E-5 2.09E-3 2.13E-3 6.94E-4 -3.73E-6 0.00E+0 -2.63E-5 -1.93E-5
POCP [kg ethene-Eq.] 2.09E-3 -3.77E-4 1.95E-4 6.29E-5 4.69E-5 -2.13E-5 4.75E-4 4.25E-4 5.76E-5 -2.49E-6 0.00E+0 -1.76E-5 -1.58E-5
ADPE [kg Sb-Eq.] 7.94E-6 1.88E-8 7.25E-7 0.00E+0 6.39E-7 1.07E-9 9.73E-8 1.07E-7 4.73E-8 -4.39E-9 0.00E+0 -3.08E-8 -4.84E-9
ADPF [MJ] 9.79E+1 2.89E+0 9.41E+0 0.00E+0 2.68E+0 1.64E-1 3.59E+0 4.22E+0 3.68E+0 -3.39E-1 0.00E+0-2.41E+0-6.24E+0
GWP = Global warming potential; ODP = Depletion potential of the stratospheric ozone layer; AP = Acidification potential of land and water; EP =
Caption Eutrophication potential; POCP = Formation potential of tropospheric ozone photochemical oxidants; ADPE = Abiotic depletion potential for non-
fossil resources; ADPF = Abiotic depletion potential for fossil resources
RESULTS OF THE LCA - INDICATORS TO DESCRIBE RESOURCE USE according to EN 15804+A1: 1 m²
floorcovering
Parameter Unit A1-A3 A4 A5 B1 B2 C2 C3/2 C3/3 C4/1 D D/1 D/2 D/3
PERE [MJ] 1.23E+2 1.62E-1 1.12E+1 0.00E+0 1.15E+0 9.17E-3 4.14E-1 6.02E-1 2.75E-1 -9.20E-2 0.00E+0 -6.43E-1 -4.64E-2
PERM [MJ] 7.30E-2 0.00E+0 -7.30E-2 0.00E+0 0.00E+0 0.00E+0 0.00E+0 0.00E+0 0.00E+0 0.00E+0 0.00E+0 0.00E+0 0.00E+0
PERT [MJ] 1.23E+2 1.62E-1 1.11E+1 0.00E+0 1.15E+0 9.17E-3 4.14E-1 6.02E-1 2.75E-1 -9.20E-2 0.00E+0 -6.43E-1 -4.64E-2
PENRE [MJ] 9.64E+1 2.90E+0 1.02E+1 0.00E+0 3.64E+0 1.65E-1 1.08E+1 1.16E+1 3.79E+0 -4.13E-1 0.00E+0 -2.93E+0 -6.26E+0
PENRM [MJ] 7.21E+0 0.00E+0 -2.41E-1 0.00E+0 0.00E+0 0.00E+0 -6.97E+0 -6.97E+0 0.00E+0 0.00E+0 0.00E+0 0.00E+0 0.00E+0
PENRT [MJ] 1.04E+2 2.90E+0 9.95E+0 0.00E+0 3.64E+0 1.65E-1 3.83E+0 4.60E+0 3.79E+0 -4.13E-1 0.00E+0 -2.93E+0 -6.26E+0
SM [kg] 3.10E+0 0.00E+0 2.79E-1 0.00E+0 0.00E+0 0.00E+0 0.00E+0 0.00E+0 0.00E+0 0.00E+0 0.00E+0 0.00E+0 2.40E-1
RSF [MJ] 0.00E+0 0.00E+0 0.00E+0 0.00E+0 0.00E+0 0.00E+0 0.00E+0 0.00E+0 0.00E+0 0.00E+0 0.00E+0 0.00E+0 0.00E+0
NRSF [MJ] 0.00E+0 0.00E+0 0.00E+0 0.00E+0 0.00E+0 0.00E+0 0.00E+0 0.00E+0 0.00E+0 0.00E+0 0.00E+0 0.00E+0 0.00E+0
FW [m³] 3.53E-1 1.85E-4 3.35E-2 0.00E+0 1.77E-3 1.05E-5 1.90E-2 1.92E-2 3.50E-5 -8.98E-5 0.00E+0 -6.28E-4 -5.09E-4
PERE = Use of renewable primary energy excluding renewable primary energy resources used as raw materials; PERM = Use of
renewable primary energy resources used as raw materials; PERT = Total use of renewable primary energy resources; PENRE = Use of
non-renewable primary energy excluding non-renewable primary energy resources used as raw materials; PENRM = Use of non-
Caption
renewable primary energy resources used as raw materials; PENRT = Total use of non-renewable primary energy resources; SM = Use
of secondary material; RSF = Use of renewable secondary fuels; NRSF = Use of non-renewable secondary fuels; FW = Use of net fresh
water
RESULTS OF THE LCA – WASTE CATEGORIES AND OUTPUT FLOWS according to EN 15804+A1:
1 m² floorcovering
Parameter Unit A1-A3 A4 A5 B1 B2 C2 C3/2 C3/3 C4/1 D D/1 D/2 D/3
HWD [kg] 8.19E-3 1.46E-10 7.37E-4 0.00E+0 6.35E-10 8.29E-12 9.31E-10 1.05E-9 6.82E-10 -9.26E-11 0.00E+0 -6.55E-10-3.98E-11
NHWD [kg] 1.12E+0 4.31E-4 1.24E-1 0.00E+0 2.59E-3 2.44E-5 2.49E-1 2.50E-1 3.62E+0 -1.92E-4 0.00E+0 -1.36E-3 -1.55E-4
RWD [kg] 2.06E-3 3.51E-6 1.94E-4 0.00E+0 3.57E-4 1.99E-7 9.55E-5 1.49E-4 4.40E-5 -2.96E-5 0.00E+0 -2.07E-4 -1.03E-5
CRU [kg] 0.00E+0 0.00E+0 0.00E+0 0.00E+0 0.00E+0 0.00E+0 0.00E+0 0.00E+0 0.00E+0 0.00E+0 0.00E+0 0.00E+0 0.00E+0
MFR [kg] 2.12E-2 0.00E+0 2.45E-2 0.00E+0 0.00E+0 0.00E+0 0.00E+0 2.40E-1 0.00E+0 0.00E+0 0.00E+0 0.00E+0 0.00E+0
MER [kg] 0.00E+0 0.00E+0 0.00E+0 0.00E+0 0.00E+0 0.00E+0 0.00E+0 0.00E+0 0.00E+0 0.00E+0 0.00E+0 0.00E+0 0.00E+0
EEE [MJ] 0.00E+0 0.00E+0 1.35E+0 0.00E+0 0.00E+0 0.00E+0 1.45E+1 0.00E+0 0.00E+0 0.00E+0 0.00E+0 0.00E+0 0.00E+0
EET [MJ] 0.00E+0 0.00E+0 2.41E+0 0.00E+0 0.00E+0 0.00E+0 2.61E+1 0.00E+0 0.00E+0 0.00E+0 0.00E+0 0.00E+0 0.00E+0
HWD = Hazardous waste disposed; NHWD = Non-hazardous waste disposed; RWD = Radioactive waste disposed; CRU = Components
Caption for re-use; MFR = Materials for recycling; MER = Materials for energy recovery; EEE = Exported electrical energy; EEE = Exported
thermal energy
References
EN 1307 CML characterization factors
DIN EN 1307: 2014+A1:2016+A2:2018-05: Textile Impact assessment characterization factors, version
floor coverings - Classification 4.7, August 2016, Institute of Environmental Sciences -
'Centrum voor Milieuwetenschappen in Leiden' (CML),
EN 13501-1 Leiden, The Netherlands
DIN EN 13501-1:2019-05: Fire classification of
construction products and building elements - Part 1:
Classification using data from reaction to fire tests ECHA candidate list
Candidate List of substances of very high concern
EN 14041 (SVHCs) for authorisation, 16.01.2020, European
DIN EN 14041: 2018-05: Resilient, textile and laminate Chemicals Agency (ECHA), Helsinki, Finland
floor coverings - Essential characteristics
ecoinvent 3.7
EN 15804 ecoinvent, Zurich, Switzerland, database version 3.7,
EN 15804:2012-04+A1 2013/, Sustainability of published September 2020
construction works — Environmental Product
Declarations — Core rules for the product category of GaBi database 2021
construction products GaBi Software-System and Database for Life Cycle
Engineering, thinkstep AG, Leinfelden-Echterdingen,
EN 16810 Database release 2021-2
DIN EN 16810: 2017-08: Resilient, textile and laminate
floor coverings – Environmental product declarations – IBU 2021
Product category rules IBU (2021): General Programme Instructions for the
Preparation of EPDs at the Institut Bauen und Umwelt
ISO 10874 e.V., Version 2.0 Institut Bauen und Umwelt e.V.,
DIN EN ISO 10874: 2012+A1:2021-04: Resilient, Berlin. www.ibu-epd.de
textile and laminate floor coverings - Classification
PCR Part A
ISO 14025 Product Category Rules for Construction Products
DIN EN /ISO 14025:2011-10/, Environmental labels from the range of Environmental Product Declarations.
and declarations — Type III environmental Part A: Calculation Rules for the Life Cycle
declarations — Principles and procedures Assessment and Requirements on the Background
Report, V1.9, Berlin: Institut Bauen und Umwelt e.V.
ISO 14040 (IBU), January 2021
DIN EN ISO 14040:2006+A1:2020 Environmental
management - Life cycle assessment - Principles and PCR Part B
framework Product Category Rules for Construction Products
from the range of Environmental Product Declarations
ISO 14044 of Institut Bauen und Umwelt (IBU),
DIN EN ISO 14044:2006+A1:2018+A2:2020 Part B: Requirements on the EPD for floor coverings,
Environmental management - Life cycle assessment - V1.2, Berlin: Institut Bauen und Umwelt e.V. (IBU),
Requirements and guidelines February 2018
ISO 15686 PRODIS
ISO 15686: Buildings and constructed assets - Product Information System (PRODIS) of the
Service life planning European Carpet Industry, Gemeinschaft
ISO 15686-1: 2011-05: Part 1: General principles and umweltfreundlicher Teppichboden e.V (GUT) and
framework European Carpet and Rug Association
ISO 15686-2: 2012-05: Part 2: Service life prediction (ECRA), http://www.pro-dis.info
procedures
ISO 15686-7: 2017-04: Part 7: Performance REACH
evaluation for feedback of service life data Regulation (EC) No 1907/2006 of the European
from practice Parliament and of the Council of 18 December 2006
ISO 15686-8: 2008-06: Part 8: Reference service life concerning the Registration, Evaluation, Authorisation
and service-life estimation and Restriction of Chemicals (REACH). Last update:
27.02.2020 (Status: 27.06.2018)
Regulation (EU) No. 305/2011
Regulation No. 305/2011 Construction Products VDZ e.V.
Regulation (CPR) of the European Council and of the Association of German Cement Works, Ed.
European Parliament, April 2011 Environmental Data of the German Cement Industry
2019
7 Environmental Product Declaration Associated Weavers Europe NV (AW) – Sedna Range - Tufted Broadloom carpet with
a pile weight of 2878 g/m2 and 100% recycled PA6 yarn
Publisher
Institut Bauen und Umwelt e.V. Tel +49 (0)30 3087748- 0
Hegelplatz 1 Fax +49 (0)30 3087748- 29
10117 Berlin Mail info@ibu-epd.com
Germany Web www.ibu-epd.com
Programme holder
Institut Bauen und Umwelt e.V. Tel +49 (0)30 - 3087748- 0
Hegelplatz 1 Fax +49 (0)30 – 3087748 - 29
10117 Berlin Mail info@ibu-epd.com
Germany Web www.ibu-epd.com
Author of the Life Cycle
Assessment Tel +49 (0)241 96843 410
Gemeinschaft umweltfreundlicher Fax +49 (0)241 96843 400
Teppichboden (GUT) e.V. Mail mail@gut-ev.de
Schönebergstraße 2 Web www.gut-ev.org
52068 Aachen
Germany
Owner of the Declaration
Associated Weavers Europe NV Tel +32 (0) 55 23 02 11
Weverijstraat 1 Fax -
9600 Ronse Mail info@awe.be
Belgium Web www.carpetyourlife.com
