ENVIRONMENTAL PRODUCT DECLARATION
as per ISO 14025 and EN 15804+A2
Owner of the Declaration ARGE – The European Federation of Locks and Building Hardware Manufacturers
Publisher Institut Bauen und Umwelt e.V. (IBU)
Programme holder Institut Bauen und Umwelt e.V. (IBU)
Declaration number EPD-ARG-20230547-IBG1-EN
Issue date 02.04.2024
Valid to 01.04.2029
Letter boxes
ARGE – The European Federation of Locks
and Building Hardware Manufacturers
This EPD is valid only for products supplied by an ARGE EPD licence holder.
www.ibu-epd.com | https://epd-online.com
1. General Information
ARGE – The European Federation of Locks Letter boxes
and Building Hardware Manufacturers
Programme holder Owner of the declaration
IBU – Institut Bauen und Umwelt e.V. ARGE – The European Federation of Locks and Building Hardware
Hegelplatz 1 Manufacturers
10117 Berlin Offerstraße 12
Germany 42551 Velbert
Germany
Declaration number Declared product / declared unit
EPD-ARG-20230547-IBG1-EN 1 kg of letter box
This declaration is based on the product category rules: Scope:
Building Hardware products, 01.08.2021 This ARGE EPD covers containers used for the receipt of mail. The
(PCR checked and approved by the SVR) reference product used to calculate the impact this product group has on
the environment is a letter box composed primarily of stainless steel and
has been selected for the LCA (Life Cycle Assessment) because it is the
Issue date product with the highest impact for 1 kg of product. A validity scope
analysis has also been carried out to determine the limiting factors for
02.04.2024
letter boxes covered by this EPD. In a preliminary study (simplified LCA), it
has been confirmed that this EPD represents the worst-case condition and
it can therefore be used to cover all letter boxes manufactured in Europe
Valid to
by ARGE member companies.
01.04.2029 The owner of the declaration shall be liable for the underlying information
and evidence; the IBU shall not be liable with respect to manufacturer
information, life cycle assessment data and evidences.
The EPD was created according to the specifications of EN 15804+A2. In
the following, the standard will be simplified as EN 15804.
Verification
The standard EN 15804 serves as the core PCR
Independent verification of the declaration and data according to ISO
14025:2011
Dipl.-Ing. Hans Peters internally X externally
(Chairman of Institut Bauen und Umwelt e.V.)
Florian Pronold Dr. Matthew Fishwick,
(Managing Director Institut Bauen und Umwelt e.V.) (Independent verifier)
1 Environmental Product Declaration - ARGE – The European Federation of Locks and Building Hardware Manufacturers - Letter boxes
2. Product
plastic substance typically derived from acrylic acid, methacrylic
2.1 Product description/Product definition
acid and acrylate monomers. Components made of Acrylic are
This EPD covers containers for the receipt and protection of formed by injection moulding or other thermal forming
letters and small parcels. processes.
For the application and use the respective national provisions
at the place of use apply. Brass is an alloy of zinc and copper. Components made of
brass are made by forging, die-casting or other types of
2.2 Application
mechanical processing.
These products are generally intended for mounting on or
within exterior walls of buildings or walls in communal areas of PC (polycarbonate) is a thermoplastic polymers containing
flats, etc. carbonate groups in its chemical structures. Components made
of PC are formed by injection moulding or other thermal forming
2.3 Technical Data
processes.
Ideally, products should comply with a suitable technical
specification. EN 13724:2013/AC:2016, Postal services –
PET (polyester) is a polymer that contains the ester functional
Apertures of private letter boxes and letter plates –
group in every repeat unit of its main chain. Components made
Requirements and test methods is an example of such a
of PET are formed by injection moulding or other thermal
specification and some products will comply with this. The
forming processes.
relevant grading structure is shown in the following table:
Name Value Unit
Steel is produced by combining iron with carbon as well as
Aperture types 1 - 4 Grade other elements depending on the desired characteristics.
Aperture sizes 1 - 3 Grade Components made of steel are formed by stamping or other
Corrosion resistance 0, 3 or 4 Grade types of mechanical processing.
Security 0, 1 or 2 Grade
Aluminium is a non-ferrous metal produced from bauxite by
the Bayer process. Components made of aluminium are
2.4 Delivery status
manufactured by extrusion or other types of mechanical
The products are sold by unit. Deliveries of individual items are processing.
possible but are an exception. Standard deliveries comprise a
larger quantity of letter boxes, as they are marketed as "B2B" 1) This product/article/at least one partial article contains
products and not to end-users. substances listed in the ECHA candidate list (date: 14.06.2023)
exceeding 0.1 percentage by mass: Certain components may
2.5 Base materials/Ancillary materials
contain small amounts of lead (CAS no. 7439-92-1) as an
Composition of product analysed for this EPD:
alloying element.
The values given in the table below are for the product
2) This product/article/at least one partial article contains other
analysed for this EPD. Ranges of values for other products
cancerogenic, mutagenic, reprotoxic (CMR) substances in
covered by the validity scope analysis are shown in brackets.
categories 1A or 1B which are not on the ECHA candidate list,
Name Value Unit exceeding 0.1 percentage by mass: no.
Stainless steel (0.06% – 90.31%) 90.31 %
Rubber (0.00% – 9.55%) 9.55 % 3) Biocide products were added to this construction product or it
has been treated with biocide products (this then concerns a
Silicone (0.00% – 0.13%) 0.13 %
treated product as defined by the (EU) Ordinance on Biocide
Acrylic (0.00% – 0.70%) 0 %
Products No. 528/2012): no.
Brass (0.00% – 3.90%) 0 %
2.6 Manufacture
PC (polycarbonate) (0.00% – 0.30%) 0 %
The production of a letter box normally follows a 3-step
PET (polyester) (0.00% – 11.14%) 0 %
procedure:
Steel (0.00% – 90.87%) 0 %
1. Manufacture of the components: this step may include
Aluminium (0.00% – 2.41%) 0 %
surface treatment in the factory or by external
contractors.
Stainless steel is produced by combining iron with chromium 2. Pre-assembly of modules (in the factory).
as well as other elements depending on the desired 3. Final assembly (in the factory).
characteristics. Components made of steel are formed by
stamping or other types of mechanical processing. 2.7 Environment and health during manufacturing
Regular measurements of air quality and noise levels are
Rubber (synthetic) is an elastomer synthesised by the carried out by the manufacturers, the ARGE member
polymerisation of petroleum byproducts. Components made of companies. The results shall be within the mandatory safety
rubber are formed by injection moulding or other thermal levels. In areas where employees are exposed to chemical
forming processes. products, the required protective clothing and technical
protective devices shall be provided. Regular health checks are
Silicone is a polymer made up of repeating units of siloxane. It mandatory for employees in production facilities.
is usually used as a sealant to prevent water penetration.
Components made of silicone are formed by injection moulding 2.8 Product processing/Installation
or other thermal forming processes. The installation of the product may vary depending on the type
of wall and the specific situation, but the products shall not
Acrylic, used in resin form, is a thermoplastic or thermosetting require energy consumption for installation.
2 Environmental Product Declaration - ARGE – The European Federation of Locks and Building Hardware Manufacturers - Letter boxes
2.9 Packaging 2.13 Extraordinary effects
Normally, each individual product is packed in cardboard. Fire
These individual products are then packed in a bigger There are no specific fire resistance requirements.
cardboard box and stacked on wooden pallets for transport to
the customer. Water
The declared product is intended to be used in buildings under
Waste from product packaging is collected separately for waste normal conditions (indoor or outdoor use). It shall not emit
disposal (including recycling). hazardous substances in the event of flooding.
2.10 Condition of use Mechanical destruction
Once installed, the products shall require no servicing during Mechanical destruction of the declared product shall not
their expected service lives. There shall be no consumption of materially alter its composition or have any adverse effect on
water or energy linked to their use, and they shall not cause the environment.
any emissions.
2.14 Re-use phase
2.11 Environment and health during use Removal of letter boxes (for re-use or recycling) shall have no
No environmental damage or health risks are to be expected adverse effect on the environment.
during normal conditions of use.
2.15 Disposal
2.12 Reference service life
Letter boxes should be recycled wherever possible, providing
The reference service life is 12 years under normal working that there is no adverse effect on the environment. The waste
conditions. This corresponds to passing a corrosion test of 384 code in accordance with the European Waste Code is 17 04 07.
hours as specified in EN 13724. The reference service life is
dependent on the actual frequency of use and environmental 2.16 Further information
conditions. It is required that installation, as well as Details of all types and variants can be found on the
maintenance of the product, must be done in line with manufacturers' websites. The respective website addresses are
instructions provided by the manufacturer. available at https://arge.org.
3. LCA: Calculation rules
European averages, with the remaining waste divided between
3.1 Declared Unit incineration and landfill. Such a mixed scenario is declared due
The declared unit for all products covered by ARGE EPD is 1 to the complex material mix of the product and the dependency
kg (of product). Since individual products will rarely weigh of the EoL-route on the EoL-route of the product the letter box
exactly 1 kg it is necessary to establish the exact weight of the has been integrated into.
product and then use this as a correction factor to determine In practice, the end of life has been modelled as follows:
the true values for 1 kg of product in the tables (Section 5).
• when a material is sent for recycling, generic transport
Declared unit and electric consumption of a shredder is taken into
Name Value Unit account (corresponding to the process 'Grinding,
metals'). Only then, is the material considered to have
Declared unit 1 kg
attained the 'end-of-waste' state.
Mass of declared product 4.54 kg
• each type of waste is modelled as a transport to the
Raw density 1 kg/m3 treatment site with a distance of 30 km. Parts sent for
recycling include electricity consumption (grinding) and
a flow ('Materials for recycling, unspecified').
3.2 System boundary
3.3 Estimates and assumptions
Type of the EPD: "cradle to gate with options, with modules C1
– C4, and module D (A1-A3, C1-C3, D and additional The LCA data of the declared product had been calculated from
modules)" the production data of 9 ARGE member companies. These
companies had been chosen by ARGE as being representative
The analysis of the product life cycle includes the production by virtue of their production processes and market share. The
and transport of the raw materials, the manufacture of the chosen product follows the "worst-case" principle as explained
product and the packaging materials which are declared in in Section 6 - LCA interpretation.
modules A1-A3.
3.4 Cut-off criteria
Losses during production are considered as waste and are sent
The cut-off criteria considered are 1% of renewable and non-
for recycling. No recycling processes are taken into account
renewable primary energy usage and 1% of the total mass of
except for transport and electricity consumption for grinding the
that unit process. The total neglected input flows per module
metals. When recycled metals are used as raw material only
shall be at a maximum of 5% of energy usage and mass.
their transformation process is taken into account and not the
extraction of the raw material.
For this study, all input and output flows have been considered
A4 module represents the transport of the finished letter box to
at 100%, including raw materials as per the product
the installation site.
composition provided by the manufacturer and packaging of
There is no waste associated with the installation of the
raw materials as well as the final product. Energy and water
product. The A5 module therefore represents only the disposal
consumption have also been considered at 100% according to
of the product packaging.
the data provided.
The End-of-Life (EoL) stages are also considered. The
transportation to the EoL disposal site is taken into account in
With the approach chosen, no significant environmental
module C2. Module C4 covers the disposal of the locks. Module
impacts are known to have been cut off.
C3 covers the recycling of the individual elements according to
3 Environmental Product Declaration - ARGE – The European Federation of Locks and Building Hardware Manufacturers - Letter boxes
3.5 Background data A total of 3 typical products (based on sales figures) have been
For the life cycle modelling of the considered product, all evaluated, and the worst-case results are used in the tables.
relevant background datasets are taken from ecoinvent v3.8
(system model: cut-off by classification). 3.7 Period under review
The data of the LCA is based on the annual production data of
3.6 Data quality an ARGE member from 2013, considered representative for the
The objective of this evaluation is to evaluate the environmental year 2022.
impacts generated by the
products throughout their entire life cycles. To this end, ISO 3.8 Geographic Representativeness
14040, ISO 14044 and EN 15804 have been met regarding the Land or region, in which the declared product system is
quality of data on the following different criteria: manufactured, used or handled at the end of the product´s
lifespan: Europe
Time: The life cycle inventory data used come from:
• Data collected specifically for this study on the ARGE
3.9 Allocation
member companies' manufacturing sites. Datasets are
The products covered by this EPD are produced on numerous
based on 1-year averaged data (time period: January
production sites. All data were provided by the manufacturers of
2013 to December 2013 considered representative for
the products by unit and then divided by the mass of the
2022).
product to give a value per kg of product produced.
• In the absence of collected data, generic data from the
ecoinvent v3.8 database have been used. This is
The assumptions relating to the EoL of the product are
updated regularly and is representative of current
described in the section System Boundaries.
processes (the entire database having been updated in
2021). 3.10 Comparability
Basically, a comparison or an evaluation of EPD data is only
Geography: Data come from production sites of the ARGE
possible if all the data sets to be compared were created
member companies. Generic data come from the ecoinvent
according to EN 15804 and the building context, respectively
database, representative for European production processes.
the product-specific characteristics of performance, are taken
into account. ecoinvent v3.8 (system model: cut-off by
Technology: Material shaping technologies are based on
classification) has been used as the background database.
European technology in the case of the use of generic data.
4. LCA: Scenarios and additional technical information
Name Value Unit
Characteristic product properties of biogenic carbon
Collected separately waste type 1 kg
Information on the biogenic carbon content at factory gate
Recycling 0.795 kg
Note: 1 kg of biogenic carbon is equivalent to 44/12 kg of CO .
2 Energy recovery 0.0943 kg
Name Value Unit Landfilling 0.111 kg
Biogenic carbon content in product 0 kg It is assumed that a 16–32-ton truck is used to transport the
C product:
Biogenic carbon content in accompanying kg - Transport to shredding facility for metal recovery: 150 km
0.0249
packaging C - Transport to municipal waste incineration plant: 50 km
- Transport to landfill: 30 km
The following information is the basis of the declared modules
within the LCA in this EPD.
Reuse, recovery and/or recycling potentials (D), relevant
Transport to the building site (A4)
scenario information
Name Value Unit
Litres of fuel 25.8 l/100km Module D contains the benefits and loads beyond the system
boundary related to the recycling of metals, which result from
Transport distance 3500 km
the treatment of recycled materials from the point of end-of-
Capacity utilisation (including empty runs) 36 %
waste status to the point of substitution (as costs) and the
substitution of primary resources (as benefits).
Installation into the building (A5)
Name Value Unit
According to EN 16710, clause 6.4.3.3: 'In module D
Material loss 0.0804 kg substitution effects are calculated only for the resulting net
output flow.
Reference service life
For building hardware, the following rules apply for the
Name Value Unit quantification of net output flows:
Reference service life 12 a - all production scrap and cuttings leave modules A1-B3 as
sorted scrap without allocated burdens from primary production;
An RSL of 12 years corresponds to passing a corrosion test of
the corresponding amounts are declared as material for
384 hours as specified in the EN 13724.
recycling (MFR);
- net amounts of a metal leaving the product system are
quantified as the material for recycling leaving modules A1-C4
End of life (C1-C4) minus the input of secondary scrap (secondary material, SM) to
4 Environmental Product Declaration - ARGE – The European Federation of Locks and Building Hardware Manufacturers - Letter boxes
the product system; quantification of module D.
- in the case of brass and zinc alloys, which are composed of
two different constituting metals, no difference shall be made It also includes the benefits and loads related to 'exported
between the input of secondary constituting metals (Cu and Zn; energy electricity' and 'exported energy heat' resulting from the
Cu and Sn) and its alloys (CuZn; CuSn). energy recovery from plastic wastes in a municipal waste
incineration plant as modelled in Modules A3, A5 and C4.
Negative net output flows have been considered in the
5 Environmental Product Declaration - ARGE – The European Federation of Locks and Building Hardware Manufacturers - Letter boxes
5. LCA: Results
In Table 1 "Description of the system boundary", the declared modules are indicated with an "X"; all modules that are not declared
within the EPD but where additional data are available are indicated with "MND". Those data can also be used for building assessment
scenarios. The values are declared with three valid digits in exponential form.
The set of characterisation factors EF3.0 has been used for the life cycle assessment.
DESCRIPTION OF THE SYSTEM BOUNDARY (X = INCLUDED IN LCA; MND = MODULE OR INDICATOR NOT DECLARED; MNR
= MODULE NOT RELEVANT)
Benefits and
Construction loads beyond
Product stage Use stage End of life stage
process stage the system
boundaries
la ire wta am R y lp p u s tro p s n a rT g n iru tc a fu n a M tro p s nm ae o rh r
T
f te tis e h t o t e ta g y lb m e s s A e s U e c n a n e tn ia M ria p e R tn e m e c a lp e R tn e m h s ib ru fe R la n o ity ag rr ee pn Oe e s u la n o ita r re et pa Ow e s u n o itc u rts n eo Dc -n o itilo m e d tro p s n a rT g n is s ee tsc ao Wrp la s o p s iD e s u e R- y re v o c e R- g n ilc y c e R- la itn e to p
A1 A2 A3 A4 A5 B1 B2 B3 B4 B5 B6 B7 C1 C2 C3 C4 D
X X X X X MND MND MNR MNR MNR MND MND X X X X X
RESULTS OF THE LCA - ENVIRONMENTAL IMPACT according to EN 15804+A2: 1 kg of letter box
Parameter Unit A1-A3 A4 A5 C1 C2 C3 C4 D
GWP-total kg CO2 eq 6.11E+00 6.16E-01 1.55E-01 0 1.22E-02 3.05E-03 1.48E-01 -1.32E+00
GWP-fossil kg CO2 eq 6.2E+00 6.16E-01 6.35E-02 0 1.22E-02 3.04E-03 1.48E-01 -1.32E+00
GWP-biogenic kg CO2 eq -9.14E-02 0 9.14E-02 0 0 0 0 0
GWP-luluc kg CO2 eq 5.48E-03 2.46E-04 6.26E-07 0 4.88E-06 7.59E-06 2.55E-06 -1.2E-03
ODP kg CFC11 eq 3.7E-07 1.43E-07 3.23E-10 0 2.83E-09 1.54E-10 1.03E-09 -6.32E-08
AP mol H+ eq 3.43E-02 1.75E-03 1.75E-05 0 3.47E-05 1.57E-05 3.87E-05 -7.62E-03
EP-freshwater kg P eq 2.48E-04 4.39E-06 2.04E-08 0 8.7E-08 3.42E-07 6.29E-08 -4.43E-05
EP-marine kg N eq 5.61E-03 3.47E-04 7.67E-06 0 6.89E-06 2.01E-06 2.02E-05 -1.24E-03
EP-terrestrial mol N eq 6.41E-02 3.87E-03 8.26E-05 0 7.68E-05 2.32E-05 1.54E-04 -1.41E-02
kg NMVOC
POCP 2.23E-02 1.49E-03 2.08E-05 0 2.95E-05 6.35E-06 4.31E-05 -4.43E-03
eq
ADPE kg Sb eq 1.55E-04 2.18E-06 6.08E-09 0 4.33E-08 7.37E-09 1.58E-08 -3.91E-05
ADPF MJ 7.63E+01 9.33E+00 2.51E-02 0 1.85E-01 6.45E-02 7.43E-02 -1.43E+01
m3 world eq
WDP 2.23E+00 2.84E-02 3.63E-04 0 5.63E-04 7.2E-04 1.11E-03 -3.69E-01
deprived
GWP = Global warming potential; ODP = Depletion potential of the stratospheric ozone layer; AP = Acidification potential of land and water; EP =
Eutrophication potential; POCP = Formation potential of tropospheric ozone photochemical oxidants; ADPE = Abiotic depletion potential for non-fossil
resources; ADPF = Abiotic depletion potential for fossil resources; WDP = Water (user) deprivation potential)
RESULTS OF THE LCA - INDICATORS TO DESCRIBE RESOURCE USE according to EN 15804+A2: 1 kg of letter box
Parameter Unit A1-A3 A4 A5 C1 C2 C3 C4 D
PERE MJ 1.47E+01 1.31E-01 -7.09E-01 0 2.6E-03 1.22E-02 2.19E-03 -3.28E+00
PERM MJ 1.01E+00 0 5.6E-01 0 0 0 0 0
PERT MJ 1.57E+01 1.31E-01 -1.48E-01 0 2.6E-03 1.22E-02 2.19E-03 -3.28E+00
PENRE MJ 7.16E+01 9.34E+00 9.26E-01 0 1.85E-01 6.51E-02 1.1E-01 -1.43E+01
PENRM MJ 4.78E+00 0 -9E-01 0 0 0 -3.53E-02 0
PENRT MJ 7.64E+01 9.34E+00 2.51E-02 0 1.85E-01 6.51E-02 7.43E-02 -1.43E+01
SM kg 5.06E-01 0 0 0 0 0 0 0
RSF MJ 0 0 0 0 0 0 0 0
NRSF MJ 0 0 0 0 0 0 0 0
FW m3 4.65E-02 9.9E-04 7.73E-05 0 1.96E-05 4.15E-05 2.01E-04 -6.25E-03
PERE = Use of renewable primary energy excluding renewable primary energy resources used as raw materials; PERM = Use of renewable primary
energy resources used as raw materials; PERT = Total use of renewable primary energy resources; PENRE = Use of non-renewable primary energy
excluding non-renewable primary energy resources used as raw materials; PENRM = Use of non-renewable primary energy resources used as raw
materials; PENRT = Total use of non-renewable primary energy resources; SM = Use of secondary material; RSF = Use of renewable secondary fuels;
NRSF = Use of non-renewable secondary fuels; FW = Use of net fresh water
RESULTS OF THE LCA – WASTE CATEGORIES AND OUTPUT FLOWS according to EN 15804+A2:
1 kg of letter box
Parameter Unit A1-A3 A4 A5 C1 C2 C3 C4 D
HWD kg 1.24E-04 2.44E-05 1.88E-07 0 4.83E-07 2.29E-08 2.13E-07 -1.06E-05
NHWD kg 7.68E+00 4.91E-01 2.49E-03 0 9.74E-03 2.42E-04 2.43E-01 -1.87E+00
RWD kg 4.18E-04 1.35E-04 2.41E-07 0 2.68E-06 8.67E-07 8.33E-07 -4.5E-05
CRU kg 0 0 0 0 0 0 0 0
MFR kg 1.78E-01 0 1.53E-02 0 0 4.56E-01 0 0
MER kg 0 0 0 0 0 0 0 0
6 Environmental Product Declaration - ARGE – The European Federation of Locks and Building Hardware Manufacturers - Letter boxes
EEE MJ 0 0 6.29E-02 0 0 0 1.5E-03 0
EET MJ 0 0 4.17E-01 0 0 0 9.92E-03 0
HWD = Hazardous waste disposed; NHWD = Non-hazardous waste disposed; RWD = Radioactive waste disposed; CRU = Components for re-use;
MFR = Materials for recycling; MER = Materials for energy recovery; EEE = Exported electrical energy; EET = Exported thermal energy
RESULTS OF THE LCA – additional impact categories according to EN 15804+A2-optional:
1 kg of letter box
Parameter Unit A1-A3 A4 A5 C1 C2 C3 C4 D
Disease
PM 4.92E-07 4.95E-08 1.77E-10 0 9.8E-10 4.19E-11 6.37E-10 -1.08E-07
incidence
IR kBq U235 eq 2.32E-01 4.05E-02 7.62E-05 0 8.03E-04 5.87E-04 2.69E-04 -2.82E-02
ETP-fw CTUe 1.89E+02 7.33E+00 3.24E-02 0 1.45E-01 3.25E-02 3.27E-01 -4.26E+01
HTP-c CTUh 1.13E-07 2.36E-10 4.16E-12 0 4.67E-12 8.67E-13 6.59E-12 -2.55E-08
HTP-nc CTUh 1.5E-07 7.4E-09 1.72E-10 0 1.47E-10 2.82E-11 1.45E-10 -3.21E-08
SQP SQP 4.1E+01 6.5E+00 1.24E-02 0 1.29E-01 9.92E-03 1.11E-01 -7.38E+00
PM = Potential incidence of disease due to PM emissions; IR = Potential Human exposure efficiency relative to U235; ETP-fw = Potential comparative
Toxic Unit for ecosystems; HTP-c = Potential comparative Toxic Unit for humans (cancerogenic); HTP-nc = Potential comparative Toxic Unit for humans
(not cancerogenic); SQP = Potential soil quality index
Disclaimer 1 –
for the indicator 'Potential Human exposure efficiency relative to U235'. This impact category deals mainly with the eventual impact of
low-dose ionizing radiation on human health of the nuclear fuel cycle. It does not consider effects due to possible nuclear accidents,
occupational exposure or radioactive waste disposal in underground facilities. Potential ionizing radiation from the soil, radon and from
some construction materials is also not measured by this indicator.
Disclaimer 2 –
for the indicators 'abiotic depletion potential for non-fossil resources', 'abiotic depletion potential for fossil resources', 'water (user)
deprivation potential, deprivation-weighted water consumption', 'potential comparative toxic unit for ecosystems', 'potential comparative
toxic unit for humans – cancerogenic', 'Potential comparative toxic unit for humans - not cancerogenic', 'potential soil quality index'. The
results of this environmental impact indicator shall be used with care as the uncertainties on these results are high as there is limited
experience with the indicator.
6. LCA: Interpretation
7 Environmental Product Declaration - ARGE – The European Federation of Locks and Building Hardware Manufacturers - Letter boxes
Figure 1 illustrates the relative contributions of the different modules along the life cycle of the declared products.
Figure 1: Environmental impacts of letter boxes along its Benefits and burdens beyond the system boundary (module D)
life cycle are in the order of 15 % to 20 % of the impacts over the product
life cycle (modules A1-A3) and relate basically to the recycling
The largest part of environmental impacts is caused during of metals.
production (modules A1-A3); comparably small impacts are
caused during the transport of the product to the construction A total of 3 typical products (based on sales figures) have been
site (via the manufacturer of the product, which the letter box evaluated and the worst-case results are used in section 5 of
has been integrated into). this EPD. In chapter 2.5, the tabulated range of relative weight
per material ensures that the variability of results stays within
All the other modules related to the product life cycle are not +/- 40% of the declared values (assessed for the indicators
significant. GWP, PENRT, and non-hazardous waste).
7. Requisite evidence
No testing results are required by the PCR part B.
8. References
Product category rules of IBU declarations - Product category rules complementary to EN
15804 for building hardware.
IBU (2021)
IBU (2021): General Instructions for the EPD Programme of the ISO 14025
Institut Bauen und Umwelt e.V. (Genera Instructions for the IBU ISO 14025:2006-07, Environmental labels and declarations -
EPD Programme). Version 2.0, Institut Bauen und Umwelt, Type III Environmental declarations - Principles and
Berlin. procedures.
IBU (2021) ISO 14044
IBU (2021): PCR Part A: Calculation rules for the life cycle EN ISO 14044:2006-07, Environmental management - Life
assessment and requirements on the project report according cycle assessment - Requirements and guidance (ISO
to EN 15804+A2. Version 1.3., Institut Bauen und Umwelt, 14044:2006).
Berlin.
EN 13724
IBU (2023) EN 13724:2013/AC:2016, Postal services – Apertures of private
IBU (2023): PCR Part B: Requirements on the EPD for building letter boxes and letter plates – Requirements and test methods.
hardware products, Institut Bauen und Umwelt, Berlin.
ISO 15686
Standards and legal documents ISO 15686:1, -2, -7 and -8. Service life planning (various parts).
EN 15804
EN 15804:2012+A2:2019+AC:2021, Sustainability of ECHA candidate list
construction works - Environmental product declarations - Core Candidate List of substances of very high concern for
rules for the product category of construction products. Authorisation, published in accordance with Article 59(10) of the
REACH Regulation. European Chemicals Agency, Brussels.
EN 17610
EN 17610:2022, Building hardware - Environmental product Ordinance on Biocide Products No. 528/2012
8 Environmental Product Declaration - ARGE – The European Federation of Locks and Building Hardware Manufacturers - Letter boxes
REGULATION (EU) No 528/2012 OF THE EUROPEAN
PARLIAMENT AND OF THE COUNCIL of 22 May 2012 Additional references
concerning the making available on the market and use of
biocidal products. BBSR 2017
BBSR (2017): Nutzungsdauer von Bauteilen in
European List of Waste Lebenszyklusanalysen nach Bewertungssystem Nachhaltiges
Commission Decision of 3 May 2000 replacing Decision Bauen (BNB). Version vom 24.10.2017, Bundesinstitut für Bau-,
94/3/EC establishing a list of wastes pursuant to Article 1(a) of Stadt- und Raumforschung, Berlin.
Council Directive 75/442/EEC on waste and Council Decision
94/904/EC establishing a list of hazardous waste pursuant to ecoinvent v3.8
Article 1(4) of Council Directive 91/689/EEC on hazardous http://www.ecoinvent.org
waste (notified under document number C(2000) 1147).
9 Environmental Product Declaration - ARGE – The European Federation of Locks and Building Hardware Manufacturers - Letter boxes
Publisher
Institut Bauen und Umwelt e.V. +49 (0)30 3087748- 0
Hegelplatz 1 info@ibu-epd.com
10117 Berlin www.ibu-epd.com
Germany
Programme holder
Institut Bauen und Umwelt e.V. +49 (0)30 3087748- 0
Hegelplatz 1 info@ibu-epd.com
10117 Berlin www.ibu-epd.com
Germany
Author of the Life Cycle Assessment
Dr. Frank Werner - Umwelt & Entwicklung + 41 (0)44 241 39 06
Kammelenbergstrasse 30 frank@frankwerner.ch
9011 St. Gallen http://www.frankwerner.ch/
Switzerland
Owner of the Declaration
ARGE – The European Federation of Locks and +49 (0)2051 9506 15
Building Hardware Manufacturers mail@arge.org
Offerstraße 12 www.arge.org
42551 Velbert
Germany
10 Environmental Product Declaration - ARGE – The European Federation of Locks and Building Hardware Manufacturers - Letter boxes
