ENVIRONMENTAL PRODUCT DECLARATION
as per ISO 14025 and EN 15804+A2
Owner of the Declaration dormakaba International Holding GmbH
Publisher Institut Bauen und Umwelt e.V. (IBU)
Programme holder Institut Bauen und Umwelt e.V. (IBU)
Declaration number EPD-DOR-20220320-CBA1-EN
Issue date 04.01.2023
Valid to 03.01.2028
BEST EHD9000
dormakaba
www.ibu-epd.com | https://epd-online.com
General Information
dormakaba BEST EHD9000
Programme holder Owner of the declaration
IBU – Institut Bauen und Umwelt e.V. dormakaba International Holding GmbH
Hegelplatz 1 DORMA Platz 1
10117 Berlin 58256 Ennepetal
Germany Germany
Declaration number Declared product / declared unit
EPD-DOR-20220320-CBA1-EN 1 door closer (1 piece) EHD9000
This declaration is based on the product category rules: Scope:
Building Hardware products, 01.08.2021 This Environment Product Declaration refers to a specific door closer
(PCR checked and approved by the SVR) manufactured by dormakaba Production GmbH & Co. KG. The production
site is located in Singapore. The data represents the year 2022.
The owner of the declaration shall be liable for the underlying information
Issue date and evidence; the IBU shall not be liable with respect to manufacturer
information, life cycle assessment data and evidences.
04.01.2023
The EPD was created according to the specifications of EN 15804+A2. In
the following, the standard will be simplified as EN 15804.
Valid to
03.01.2028 Verification
The standard EN 15804 serves as the core PCR
Independent verification of the declaration and data according to ISO
14025:2011
internally X externally
Dipl.-Ing. Hans Peters
(Chairman of Institut Bauen und Umwelt e.V.)
Florian Pronold Dr.-Ing. Wolfram Trinius,
(Managing Director Institut Bauen und Umwelt e.V.) (Independent verifier)
1 Environmental Product Declaration - dormakaba - BEST EHD9000
Product
Product description/Product definition Base materials/Ancillary materials
The EHD9000 is a cast iron closer for all institutional Name Value Unit
applications. It comes with self-regulating valves that
Steel 44 %
significantly reduces the need to adjust the door closer in
Aluminum 39 %
fluctuating temperatures and high-traffic areas. Front-facing
Paper 11 %
spring force adjustment including spring-size indicator, and
valves for adjustment of hydraulic functions. It utilizes a robust Plastic 3 %
dual clamp fit cover design that strongly secures the cover on Others (Lacquer) 2 %
both ends. For the use and application of the product the
The product/s include/s partial articles which contain
respective national provisions at the place of use apply. The
substances listed in the Candidate List of REACH Regulation
EHD9000 is a Underwriters Laboratories (UL) listed product.
1907/2006/EC (date: 10.06.2022) exceeding 0.1 percentage by
The standards which can be applied are the following:
mass: yes
• ANSI/BHMA 156.4
• Lead (Pb): 7439-92-1 (CAS-No.) is included in some of
• ANSI/ICC A117.1
the alloys used. The concentration of lead in each
• UL 10C
individual alloy does not exceed 4.0% (by mass).
• ADA
The Candidate List can be found on the ECHA website
Application address: https://echa.europa.eu/de/home.
The EHD9000 series closers are designed for commercial and
Reference service life
institutional applications, including ADA barrier-free accessibility
The reference service life of the EHD9000 depends on the
requirements. They are suitable for use on hollow metal,
traffic pattern and degree of usage of the door. These closers
aluminum and wood doors and can be used for fire doors.
are rated to ANSI Grade 1, meaning they are designed to
Technical Data withstand a minimum of 1,500,000 cycles. The reference
service life amounts for 20 years.
Performance data of the product with respect to its
characteristics in accordance with the relevant technical
provision which can be applied are mentioned above.
LCA: Calculation rules
Declared unit
Declared Unit
The declared unit is 1 piece of the product: EHD 9000. Name Value Unit
Declared unit 1 piece/product
Mass of declared Product 7.25 kg
2 Environmental Product Declaration - dormakaba - BEST EHD9000
— C1, de-construction, demolition:
System boundary — C2, transport to waste processing;
The type of EPD is: cradle to gate with options, modules C1– — C3, waste processing for reuse, recovery and/or recycling;
C4, and module D (A1–A3 + C + D and additional modules: A4 — C4, disposal;
+ A5) including provision and all transport, provision of all materials,
products and related energy and water use.
Production - Module A1-A3
The product stage includes:
— A1, raw material extraction, processing and mechanical Module D (Benefits and loads beyond the system boundary)
treatments, processing of secondary material input (e.g. includes:
recycling processes), — A2, transport to the manufacturer, — D, recycling potentials, expressed as net impacts and
— A3, manufacturing and assembly including provision of all benefits.
materials, products and energy, as well as waste processing up
to the end-of waste state. Geographic Representativeness
Land or region, in which the declared product system is
Construction stage - Modules A4-A5 manufactured, used or handled at the end of the product´s
The construction process stage includes: lifespan: Singapore
— A4, transport to the building site;
— A5, installation into the building;
Comparability
including provision of all materials, products and energy, as well
as waste processing up to the end-of waste state or disposal of Basically, a comparison or an evaluation of EPD data is only
final residues during the construction process stage. possible if all the data sets to be compared were created
according to EN 15804 and the building context, respectively
End-of-life stage– Modules C1-C4 and D the product-specific characteristics of performance, are taken
The end-of-life stage includes: into account.
LCA: Scenarios and additional technical information
Installation into the building (A5)
Characteristic product properties of biogenic carbon
Name ValueUnit
Information on describing the biogenic Carbon Content at
Output substances following waste treatment on
factory gate 0.76 kg
site (paper packaging)
Name ValueUnit
Output substances following waste treatment on
kg 0,007 kg
Biogenic carbon content in product 0.01 site (plastic packaging)
C
Biogenic carbon content in accompanying kg End of life (C1-C4)
0.28
packaging C C1: The product dismantling from the building is done manually
without environmental burden.
Note: 1 kg of biogenic carbon is equivalent to 44/12 kg of CO .
2 C2: Transport to waste treatment at end of life is 50km.
Name Value Unit
Additional technical information for the Collected separately waste type 6.49 kg
declared modules. Recycling 6.28 kg
Transport to the building site (A4) Energy recovery 0.205 kg
Name Value Unit
Reuse, recovery and/or recycling potentials (D), relevant
Litres of fuel per 1 kg (truck) 0.00276l/100km
scenario information
Transport distance via truck 100 km
Name Value Unit
Capacity utilisation (including empty runs)
55 % Recycling 100 %
average
Collection rate is 100%.
Transport distance via ship 22000 km
The product is transported via truck and ship. The main
distribution regions are the USA and Dubai. In order to allow
scaling to a specific point of installation via truck, 100 km are
declared.
3 Environmental Product Declaration - dormakaba - BEST EHD9000
LCA: Results
DESCRIPTION OF THE SYSTEM BOUNDARY (X = INCLUDED IN LCA; MND = MODULE OR INDICATOR NOT DECLARED; MNR
= MODULE NOT RELEVANT)
Benefits and
Construction loads beyond
Product stage Use stage End of life stage
process stage the system
boundaries
la ire ta m w a Ry lp p u s tro p s n a rT g n iru tc a fu n a M e h t m o rf tro p s n a rTe tis e h t o t e ta g y lb m e s s A e s U e c n a n e tn ia M ria p e R tn e m e c a lp e R tn e m h s ib ru fe R y g re n e la n o ita re p Oe s u re ta w la n o ita re p Oe s u n o itc u rts n o c -e Dn o itilo m e d tro p s n a rT g n is s e c o rp e ts a W la s o p s iD -e s u e R-y re v o c e R-g n ilc y c e Rla itn e to p
A1 A2 A3 A4 A5 B1 B2 B3 B4 B5 B6 B7 C1 C2 C3 C4 D
X X X X X MND MND MNR MNR MNR MND MND X X X X X
RESULTS OF THE LCA - ENVIRONMENTAL IMPACT according to EN 15804+A2: 1 door closer
Parameter Unit A1-A3 A4 A5 C1 C2 C3 C4 D
GWP-total kg CO 2 eq 7.3E+01 5.85E-01 1.09E+00 0 2.84E-02 1.03E+00 0 -1.97E+01
GWP-fossil kg CO 2 eq 7.42E+01 5.81E-01 4.6E-02 0 2.71E-02 9.75E-01 0 -1.96E+01
GWP-biogenic kg CO 2 eq -1.27E+00 3.48E-03 1.04E+00 0 1.25E-03 5.8E-02 0 -6.12E-02
GWP-luluc kg CO 2 eq 2.11E-02 1.22E-05 1.87E-05 0 6.45E-07 5.57E-05 0 -3.09E-03
ODP kg CFC11 eq 5.57E-10 5.56E-17 2.03E-16 0 2.86E-18 4.99E-16 0 -1.47E-10
AP mol H+ eq 3.91E-01 1.93E-02 3.04E-04 0 2.71E-05 1.82E-04 0 -7.16E-02
EP-freshwater kg P eq 4.19E-05 1.3E-07 3.93E-08 0 5.8E-09 7.95E-08 0 -1.03E-05
EP-marine kg N eq 6.01E-02 5.09E-03 1.09E-04 0 8.64E-06 4.19E-05 0 -9.55E-03
EP-terrestrial mol N eq 6.52E-01 5.58E-02 1.37E-03 0 9.6E-05 8.3E-04 0 -1.03E-01
kg NMVOC
POCP 1.86E-01 1.42E-02 2.89E-04 0 2.44E-05 1.16E-04 0 -3.05E-02
eq
ADPE kg Sb eq 3.16E-04 1.52E-08 3.18E-09 0 8.13E-10 6.85E-09 0 -2.88E-05
ADPF MJ 7.21E+02 7.17E+00 3.47E-01 0 3.85E-01 4.64E-01 0 -2.78E+02
m3 world eq
WDP 1.15E+01 1.06E-03 1.35E-01 0 5.31E-05 1.06E-01 0 -9.25E-01
deprived
GWP = Global warming potential; ODP = Depletion potential of the stratospheric ozone layer; AP = Acidification potential of land and water; EP =
Eutrophication potential; POCP = Formation potential of tropospheric ozone photochemical oxidants; ADPE = Abiotic depletion potential for non-fossil
resources; ADPF = Abiotic depletion potential for fossil resources; WDP = Water (user) deprivation potential)
RESULTS OF THE LCA - INDICATORS TO DESCRIBE RESOURCE USE according to EN 15804+A2: 1 door closer
Parameter Unit A1-A3 A4 A5 C1 C2 C3 C4 D
PERE MJ 7.08E+01 2.34E-02 9.14E+00 0 1.21E-03 5.08E-01 0 -1.26E+02
PERM MJ 9.46E+00 0 -9.07E+00 0 0 -3.88E-01 0 0
PERT MJ 8.03E+01 2.34E-02 6.38E-02 0 1.21E-03 1.2E-01 0 -1.26E+02
PENRE MJ 7.13E+02 7.17E+00 6.71E-01 0 3.85E-01 8.36E+00 0 -2.78E+02
PENRM MJ 8.22E+00 0 -3.23E-01 0 0 -7.89E+00 0 0
PENRT MJ 7.21E+02 7.17E+00 3.47E-01 0 3.85E-01 4.65E-01 0 -2.78E+02
SM kg 2.7E+00 0 0 0 0 0 0 0
RSF MJ 0 0 0 0 0 0 0 0
NRSF MJ 0 0 0 0 0 0 0 0
FW m3 2.9E-01 4.25E-05 3.18E-03 0 2.18E-06 2.53E-03 0 -2.21E-01
PERE = Use of renewable primary energy excluding renewable primary energy resources used as raw materials; PERM = Use of renewable primary
energy resources used as raw materials; PERT = Total use of renewable primary energy resources; PENRE = Use of non-renewable primary energy
excluding non-renewable primary energy resources used as raw materials; PENRM = Use of non-renewable primary energy resources used as raw
materials; PENRT = Total use of non-renewable primary energy resources; SM = Use of secondary material; RSF = Use of renewable secondary fuels;
NRSF = Use of non-renewable secondary fuels; FW = Use of net fresh water
RESULTS OF THE LCA – WASTE CATEGORIES AND OUTPUT FLOWS according to EN 15804+A2:
1 door closer
Parameter Unit A1-A3 A4 A5 C1 C2 C3 C4 D
HWD kg 2.07E-05 7.04E-10 5.33E-10 0 3.73E-11 1.73E-09 0 -1.5E-06
NHWD kg 1.16E+01 7.35E-04 3.56E-02 0 3.94E-05 1.02E-01 0 -4.77E+00
RWD kg 5.2E-03 7.97E-06 1.81E-05 0 4.13E-07 1.75E-05 0 -3.03E-02
CRU kg 0 0 0 0 0 0 0 0
MFR kg 0 0 0 0 0 6.07E+00 0 0
MER kg 0 0 0 0 0 0 0 0
EEE MJ 0 0 1.66E+00 0 0 0 0 0
EET MJ 0 0 3.02E+00 0 0 0 0 0
HWD = Hazardous waste disposed; NHWD = Non-hazardous waste disposed; RWD = Radioactive waste disposed; CRU = Components for re-use;
MFR = Materials for recycling; MER = Materials for energy recovery; EEE = Exported electrical energy; EET = Exported thermal energy
4 Environmental Product Declaration - dormakaba - BEST EHD9000
RESULTS OF THE LCA – additional impact categories according to EN 15804+A2-optional:
1 door closer
Parameter Unit A1-A3 A4 A5 C1 C2 C3 C4 D
Disease
PM 1.12E-05 3.28E-07 1.71E-09 0 1.43E-10 2.26E-09 0 -1.15E-06
incidence
IR kBq U235 eq 6.26E-01 1.14E-03 2.78E-03 0 5.9E-05 1.62E-03 0 -6.08E+00
ETP-fw CTUe 2.48E+02 5.07E+00 1.64E-01 0 2.73E-01 1.75E-01 0 -1E+02
HTP-c CTUh 2.67E-08 9.55E-11 8.78E-12 0 5.13E-12 1.5E-11 0 -4.45E-09
HTP-nc CTUh 8.46E-07 4.48E-09 3.97E-10 0 2.19E-10 1.5E-09 0 -1.4E-07
SQP SQP 1.87E+02 1.9E-02 9.24E-02 0 9.88E-04 1.39E-01 0 -8.68E+00
PM = Potential incidence of disease due to PM emissions; IR = Potential Human exposure efficiency relative to U235; ETP-fw = Potential comparative
Toxic Unit for ecosystems; HTP-c = Potential comparative Toxic Unit for humans (cancerogenic); HTP-nc = Potential comparative Toxic Unit for humans
(not cancerogenic); SQP = Potential soil quality index
Disclaimer 1 – for the indicator “Potential Human exposure efficiency relative to U235”. This impact category deals mainly with the
eventual impact of low-dose ionizing radiation on human health of the nuclear fuel cycle. It does not consider effects due to possible
nuclear accidents, occupational exposure or radioactive waste disposal in underground facilities. Potential ionizing radiation from the
soil, radon and from some construction materials is also not measured by this indicator.
Disclaimer 2 – for the indicators “abiotic depletion potential for non-fossil resources”, “abiotic depletion potential for fossil resources”,
“water (user) deprivation potential, deprivation-weighted water consumption”, “potential comparative toxic unit for ecosystems”,
“potential comparative toxic unit for humans – cancerogenic”, “Potential comparative toxic unit for humans - not cancerogenic”,
“potential soil quality index”. The results of this environmental impact indicator shall be used with care as the uncertainties on these
results are high as there is limited experience with the indicator.
References
ADA (version 1-6) Further References
Americans with Disabilities Act 1990
IBU
ANSI/ICC A117.1 Institut Bauen und Umwelt e.V.: General Instructions for the
ANSI/ICC A117.1:2017, Accessible and usable buildings and EPDs programme of Institut Bauen und Umwelt e.V. Version
facilities 2.0., Berlin: Institut Bauen und Umwelt e.V., 2021. www.ibu-
epd.com
ANSI/BHMA A156.4
ANSI/BHMA A156.4:2019, Door controls — Closers GaBi
Sphera Solutions GmbH
Candidate List of REACH Regulation /1907/2006/EC (date: Gabi Software System and Database for Life Cycle Engineering
16.01.2020) 1992-2020 Version 10.0.0.71
ECHA GaBi ts documentation
European Chemicals Agency: https://echa.europa.eu/de/home GaBi life cycle inventory data documentation
(https://www.gabi-software.com/support/gabi/gabidatabase-
UL 10C 2020-lci-documentation/)
UL 10C:2016, Positive pressure fire tests of door assemblies
LCA-tool dormakaba
REACH LCA tool IBU-DOR-202104-LT1-EN, version 1.0, 2021.
Registration, Evaluation, Authorisation and Restriction of Developed by Sphera Solutions GmbH
Chemicals (REACH), Regulation (EC) No 1907/2006
PCR Part A
EN 15804 PCR – Part A: Calculation Rules for the Life Cycle Assessment
EN 15804+A2:2019+A2+AC:2021, Sustainability of and Requirements on the Project Re-port according to EN
construction works — Environmental Product Declarations — 15804+A2:2019, Version 1.0, 2020, Institut Bauen und Umwelt
Core rules for the product category of construction products e.V., www.ibu-epd.com
ISO 14025 PCR Part B
DIN EN ISO 14025:201110, Environmental labels and PCR – Part B: Requirements on the EPD for Building
declarations — Type III environmental declarations — Hardware product, version 1.2, Institut Bauen und
Principles and procedures Umwelt e.V., www.ibu-epd.com, 2017
5 Environmental Product Declaration - dormakaba - BEST EHD9000
Publisher
Institut Bauen und Umwelt e.V. +49 (0)30 3087748- 0
Hegelplatz 1 info@ibu-epd.com
10117 Berlin www.ibu-epd.com
Germany
Programme holder
Institut Bauen und Umwelt e.V. +49 (0)30 3087748- 0
Hegelplatz 1 info@ibu-epd.com
10117 Berlin www.ibu-epd.com
Germany
Author of the Life Cycle Assessment
Sphera Solutions GmbH +49 711 341817-0
Hauptstraße 111- 113 info@sphera.com
70771 Leinfelden-Echterdingen www.sphera.com
Germany
Owner of the Declaration
dormakaba International Holding GmbH +49 2333 793-0
DORMA Platz 1 info.de@dormakaba.com
58256 Ennepetal www.dormakaba.com
Germany
6 Environmental Product Declaration - dormakaba - BEST EHD9000
