ENVIRONMENTAL PRODUCT DECLARATION
as per ISO 14025 and EN 15804+A2
Owner of the Declaration DBC, EFCC, FEICA, IVK
Programme holder Institut Bauen und Umwelt e.V. (IBU)
Publisher Institut Bauen und Umwelt e.V. (IBU)
Declaration number EPD-DBC-20220179-IBF1-EN
Issue date 31.08.2022
Valid to 30.08.2027
Silicone-based products, group 1
DBC - Deutsche Bauchemie e.V.
EFCC - European Federation for Construction Chemicals
FEICA - Association of the European Adhesive and Sealant Industry
IVK - Industrieverband Klebstoffe e.V.
www.ibu-epd.com | https://epd-online.com
Umwelt Produktdeklaration Name des Herstellers – Name des Produkts
1. General Information
DBC - Deutsche Bauchemie e.V. Silicone-based products, group 1
EFCC - European Federation for
Construction Chemicals
FEICA - Association of the European
Adhesive and Sealant Industry
IVK - Industrieverband Klebstoffe e.V.
Programme holder Owner of the declaration
IBU – Institut Bauen und Umwelt e.V. DBC, Mainzer Landstr. 55, D-60329 Frankfurt a.M.
Panoramastr. 1 EFCC, 172 Boulevard du Triomphe, B-1160 Brussels
10178 Berlin FEICA, Rue Belliard 40, B-1040 Brussels
Germany IVK, Völklingerstr. 4, D-40219 Düsseldorf
Declaration number Declared product / declared unit
EPD-DBC-20220179-IBF1-EN 1 kg silicone-based product, group 1; density 1.0 - 1.5
g/cm³
This declaration is based on the product Scope:
category rules: This verified EPD entitles the holder to bear the
Building sealants, 07.2014 symbol of the Institut Bauen und Umwelt e.V. It
(PCR checked and approved by the SVR) exclusively applies for products produced in Europe
and for a period of five years from the date of issue.
This EPD may be used by members of DBC, EFCC,
Issue date
FEICA and IVK and their members provided it has
31.08.2022
been proven that the respective product can be
represented by this EPD. For this purpose, a guideline
Valid to is available at the secretariats of the four associations.
30.08.2027 The members of the associations are listed on their
respective websites.
The owner of the declaration shall be liable for the
underlying information and evidence; the IBU shall not
be liable with respect to manufacturer information, life
cycle assessment data and evidences.
The EPD was created according to the specifications
of EN 15804+A2. In the following, the standard will be
simplified as EN 15804.
Verification
The standard EN 15804 serves as the core PCR
Independent verification of the declaration and data
according to ISO 14025:2010
Dipl. Ing. Hans Peters internally x externally
(chairman of Institut Bauen und Umwelt e.V.)
Dr. Alexander Röder Matthias Schulz
(Managing Director Institut Bauen und Umwelt e.V.)) (Independent verifier)
2. Product
2.1 Product description/Product definition based products fulfil key functions. Ingress of moisture
Silicone-based products, group 1 with a Volatile into the structure via the joints is prevented by joint
Organic Compound (VOC) content ≤2 % (VOC sealants. With the use of silicone-based products, the
definition according to Decopaint Directive) are fitness for use of the building and the service life are
manufactured from reactive siloxane and so-called decisively extended. The product displaying the
silicone oil, optionally by using fillers, extenders, colour highest environmental impacts was used as a
pigments, cross-linkers, bonding agents and catalysts. representative product for calculating the Life Cycle
For most of the applications the products are Assessment results (worst-case approach).
formulated as moisture-reactive one-component For the placing on the market in the European
systems; for industrial applications there are also two- Union/European Free Trade Association (EU/EFTA)
component systems available. They permanently and with the exception of Switzerland) products falling
elastically seal joints planned for the building. Silicone- under the Regulation (EU) No 305/2011 (CPR) need a
2 Environmental Product Declaration DBC, EFCC, FEICA, IVK – Silicone-based products, group 1
Declaration of Performance taking into consideration
either the relevant harmonised European standard or Constructional data
the European Technical Assessment and the CE Name Value Unit
marking. For the application and use of the products only for
the respective national provisions apply. module 2:
Elastic recovery EN ISO 7389 %
>/=25 or
2.2 Application >/=100
Module 1: Façade sealants value to be
Silicone-based products are used for the elastic declared
sealing of joints. The areas of application for façade Loss of volume EN ISO 10563 by the %
sealants include expansion joints (movement joints) manufactur
and/or connection joints already existing in exterior er
walls and on window and door frames (including the only for
inside section). All these sealants fulfil key functions of module 1,2
the building. and 3;
value to be
Resistance to flow EN ISO 7390 mm
Module 2: Sealants for glazing declared
Silicone-based products are used for the elastic by the
sealing of joints which may be subject to movement. manufactur
Sealants for glazing are used in the following areas: er
(i)Glass to glass (ii)Glass to frame (iii)Glass to porous only for
substrates module 1,
Tensile properties EN ISO 8339
3 and 4:
Module 3: Sanitary sealants </=0,9
The areas of application for silicone-based sanitary Adhesion/cohesion properties at only for
sealants are joints in sanitary areas and kitchens. maintained extension after module 1
Joints sealed using sanitary sealants comprise immersion in water EN ISO 10590 and 4: NF*
connection joints between sanitary furnishings and the only for
wall, connection joints between the floor and wall or Adhesion/cohesion properties module 1:
movement joints across surfaces, for example. after immersion in water plastic >/=25 or %
sealants EN ISO 10591
>/=100
Module 4: Sealants for pedestrian walkways Adhesion/cohesion properties only for
The areas of application for silicone-based sealants for after exposure to heat, water and module
pedestrian walkways are floor joints designed for artificial light EN ISO 11431 2:NF*
pedestrian walkways, public areas, movement joints
Adhesion/cohesion properties at
between concrete slabs, areas with pedestrian load,
maintained extension after
areas used with trolleys, walkable floors, balconies,
immersion in water for sealants in only for
terraces, warehouses.
class XS and/or module 3
adhesion/cohesion properties after and 4: NF*
Module 5: Bonded glazing sealants
immersion in water for sealants in
One- and two-component structural sealants are to be
class S EN ISO 10590
used in a structural sealant glazing system (SSGK) to
Adhesion/cohesion properties at only for
bond glazing products to metallic structural seal
maintained extension after 28 module
support frames and/or as the second barrier of the
days salt water immersion 4**: NF*
structural hermetic seal in insulating glass units.
* NF: Passed-Failed criteria. The sealant class must
also be indicated for the declared product.
2.3 Technical Data
** not required for interior use
The density of the products is between 1,00 and 1,50
valid for all modules: Other performance
g/cm³, other relevant technical data can be found in the
characteristics in accordance with the manufacturer's
manufacturer’s technical documentation.
technical documentation/declaration of performance
Module 1: Façade sealants
The minimum requirements on water and airtightness
as per Table ZA.1 of EN 15651-1 apply: see table
2.4 Delivery status
Module 2: Sealants for glazing
Pasty in containers made of plastic, foil or metal.
The minimum requirements on water and airtightness
Typical container sizes contain 50 ml to 1000 ml of
as per Table ZA.1 of EN 15651- 2 apply: see table
product. A combination of HDPE (high-density
polyethylene) cartridges, cardboard and pallets was
Module 3: Sanitary sealants
modelled for the LCA. For one and two component
The minimum requirements on water and airtightness
bonded glazing sealants (Module 5) 200 l metal drums
as per Table ZA.1 of EN 15651-3 apply: see table
and plastic or metal 20 l pails are used as containers.
Module 4: Sealants for pedestrian walkways
2.5 Base materials/Ancillary materials
The minimum requirements on water and airtightness
Silicone-based products, group 1 are manufactured
as per Table ZA.1 of EN 15651-4 apply: see table
from reactive siloxane and silanes, sometimes using
fillers. The cross-linking reaction occurs through the
Module 5: Bonded glazing sealants
effects of humidity in the air when installed. Typically,
Structural Sealants must comply with ETAG 002-
the products covered by this EPD contain the following
1 used as EAD.
range of base materials and auxiliaries (% by mass):
3 Environmental Product Declaration DBC, EFCC, FEICA, IVK – Silicone-based products, group 1
Siloxanes: 45-90 consistently adhered to in accordance with the
Silanes: 2-10 information on the safety data sheet and conditions on
Silicone plasticizers: 0-30 site. VOC emissions may occur. Two-component
Mineral fillers: 0-50 silicone products are processed on the job site by
Fumed silica: 0-20 using mix cartridges with static mixers. On the shop
Mineral oil/Solvent: 0-30 floor, two-component dosing & mixing equipment is
Pigments: 0-20 used (static or dynamic mixers) and the mixed product
Water: 0-20 can be applied manually or fully automatically by a
Additives: <5 sealing robot.
VOC according to Decopaint Directive: ≤2 %
(mandatory) 2.9 Packaging
A detailed description of packaging is provided in
These ranges are average values and the composition section 2.4. Empty containers and clean foils can be
of products complying with the EPD can deviate from recycled.
these concentration levels in individual cases. More
detailed information is available in the respective
manufacturer's documentation (e.g. product data 2.10 Condition of use
sheets). During the use phase, silicone-based products are fully
cross-linked and hardened. They are durable products
Note: For companies to declare their products within which protect buildings and significantly contribute
the scope of this EPD it is not sufficient to simply towards their appearance, function and long-term
comply with the product composition shown above. value.
The application of this EPD is only possible for
member companies of DBC, EFCC, FEICA, and IVK 2.11 Environment and health during use
member associations and only for specific formulations Option 1 – Products for applications outside
with a total score below the declared maximum score indoor areas with permanent stays by people
for a product group according to the associated During use, silicone-based products lose their reactive
guidance document. capacity and are inert. No risks are known for water,
air and soil if the products are used as designated.
1. substances from the “Candidate List of
Substances of Very High Concern for Option 2 – Products for applications inside indoor
Authorisation” (SVHC) areas with permanent stays by people
If this product contains substances listed in the When used in indoor areas with permanent stays by
candidate list (latest version) exceeding 0.1 people, evidence of the emission performance of
percentage by mass, the relevant information can be construction products in contact with indoor air must be
found in the safety data sheet of the relevant product submitted according to national requirements. No
covered by this model EPD. further influences on the environment and health by
2. CMR substances in categories 1A and 1B emanating substances are known.
If this product contains other carcinogenic, mutagenic,
reprotoxic (CMR) substances in categories 1A or 1B 2.12 Reference service life
which are not on the candidate list, exceeding 0.1 Sealants fulfil key functions in buildings. They
percentage by mass, the relevant information can be decisively improve the usability of building structures
found in the safety data sheet of the relevant product and significantly extend their original service lives.
covered by this model EPD. Information supplied by the manufacturer on
3. Biocide products added to the construction maintenance and care must be observed.
product
If this construction product contains biocide products,
the active substances, information on the 2.13 Extraordinary effects
concentration and/or concentration range, the product
type together with information on their hazardous Fire
properties are listed in the safety data sheet of the Even without any special fire safety features, joint
respective product. sealants comply with at least the requirements of EN
13501-1 for fire class E. In terms of volumes used,
sealants generally have no or only a minor influence
2.6 Manufacture on the fire characteristics (e.g. smoke gas
Silicone-based products are generally manufactured development) of the building in which they are
by mixing the ingredients and then filling them into the applied.
delivery containers.
Water
2.7 Environment and health during Silicone-based products are insoluble in water. They
manufacturing are often used to protect building structures from
As a general rule, no other environmental or health harmful water ingress or the effects of flooding.
protection measures other than those specified by law
are necessary. Mechanical destruction
The mechanical destruction of silicone-based products
2.8 Product processing/Installation does not lead to any decomposition products which are
One-component silicone-based products are usually harmful to the environment or health.
processed manually on site using suitable tools. In
most cases, the products are inserted into joints using 2.14 Re-use phase
cartridge guns, whereby health and safety measures According to present knowledge, no environmentally
(gloves and goggles, ventilation) are to be taken and hazardous effects in terms of landfilling are to be
4 Environmental Product Declaration DBC, EFCC, FEICA, IVK – Silicone-based products, group 1
generally anticipated through dismantling and recycling commercial/site waste. The following waste codes
of components to which hardened silicone sealants according to the European List of Waste (EWC)
adhere. (2000/532/EC) can apply:
Product residue: EWC 08 04 09
2.15 Disposal EWC 08 04 10 with the exception of those covered by
Silicone-based products which cannot be recycled can EWC 08 04 09
be hardened. Empty containers are directed to the
recycling process. Only a low volume of silicone 2.16 Further information
sealants is incurred in the disposal of components in More information is available on the manufacturer's
which they are used. Low levels of adhesion do not product or safety data sheets and is available on the
play any role in terms of disposal. They do not impair manufacturer's websites or on request. Valuable
the disposal/recycling of other components/building technical information is also available on the
materials. Hardened residual product mechanically associations' websites.
removed from substrates must be disposed of as
3. LCA: Calculation rules
3.1 Declared Unit processes are considered. For precautionary principle
This EPD refers to the declared unit of 1 kg of silicone- and as a worst-case scenario, thermal treatment is the
based product, group 1; applied into the building with a only end-of-life scenario considered. This is modelled
density of 1.0 - 1.5 g/cm³ in accordance with the IBU by the incineration process (module C3) where the
PCR part B for construction sealants. product ends its life cycle.
The results of the Life Cycle Assessment provided in Module D accounts for potential benefits that are
this declaration have been selected from the product beyond the defined system boundaries. Credits are
with the highest environmental impact (worst-case generated during the incineration of wastes and related
scenario). electricity produced that are occurring in the A5
Depending on the application, a corresponding module.
conversion factor such as the density to convert
volumetric use to mass must be taken into 3.3 Estimates and assumptions
consideration. For this EPD formulation and production data defined
and collected by FEICA were considered. Production
The Declaration type is according to EN 15804: Cradle waste was assumed to be disposed of by incineration
to gate with options, modules C1–C3, and module D without credits as a worst-case for recovered thermal
(A1–A3, C, D) and additional modules (A4-A5). energy (recovered electricity is looped back within
module A1-A1).
Declared unit An average of plastic containers and wooden pallets
Name Value Unit was considered in the LCA.
Declared unit 1 kg
Gross density 1-1.5 g/cm^3 3.4 Cut-off criteria
All raw materials submitted for the formulations and
production data were taken into consideration.
The manufacture of machinery, plant and other
3.2 System boundary infrastructure required for the production of the
Modules A1, A2 and A3 are taken into consideration in products under review was not taken into consideration
the LCA: in the LCA.
- A1 Production of preliminary products Transport of packaging materials is excluded.
- A2 Transport to the plant
- A3 Production incl. provision of energy, production of 3.5 Background data
packaging as well as auxiliaries and consumables and Data from the GaBi database SP40 (2020) was used
waste treatment as background data.
- A4 Transport to site
- A5 Installation, product applied into the building 3.6 Data quality
during A5 phase operations and packaging Representative products were applied for this EPD and
disposal. This stage considers VOC emissions during the product in the group displaying the highest
the installation phase. The declared product does not environmental impact was selected for calculating the
contain substances in(to) the formulation that directly LCA results. The background datasets used are less
emit as VOC, but VOCs are generated by a chemical than 4 years old.
reaction that is occurring during this phase. Production data and packaging are based on details
The end of life for the packaging material considered is provided by the manufacturer. The formulation used for
described below: evaluation refers to a specific product.
-Incineration, for materials like plastic, paper and The data quality of the background data is considered
wood. to be good.
-C1-C2-C3-D
The building deconstruction (demolition process) takes 3.7 Period under review
place in the C1 module which considers energy Representative formulations are valid for 2021.
generation and consumption of diesel and all the
emissions connected with the fuel-burning process to 3.8 Allocation
run the machines. After the demolition, the product is Mass allocation has been applied when primary data
transported to the end-of-life processing (C2 module) have been used and implemented into the LCA model.
where all the impacts related to the transport
5 Environmental Product Declaration DBC, EFCC, FEICA, IVK – Silicone-based products, group 1
3.9 Comparability context, respectively the product-specific
Basically, a comparison or an evaluation of EPD data characteristics of performance, are taken into account.
is only possible if all the data sets to be compared
were created according to EN 15804 and the building The GaBi database SP40 (2020) was used.
4. LCA: Scenarios and additional technical information
Characteristic product properties
Information on biogenic Carbon
The packaging material contains biogenic carbon
which is presented below.
Information on describing the biogenic Carbon
Content at factory gate
Name Value Unit
Biogenic Carbon Content in
- kg C
product
Biogenic Carbon Content in
0.024 kg C
accompanying packaging
For the preparation of building life cycle assessments,
it must be taken into account that in module A5
(installation in the building) the biogenic amount of CO
2
(0.024 kg C *3.67 = 0.088 kg CO -eq.) of the
2
packaging bound in module A1-A3 is mathematically
booked out.
Transport to the building site (A4)
Name Value Unit
Transport distance 1000 km
Gross weight 34 - 40 t
Payload capacity 27 t
Installation into the building (A5)
Name Value Unit
Other resources for packaging
0.225 kg
material
Material loss 0.01 kg
Material loss considers the amount of product not used
during the application phase into the building. This
amount is 1 % of the product and, impacts related to
the production of this part are assigned to the A5
module. This percentage is considered as waste to
disposal and impacts of its end of life have been
considered in the LCA model and declared in A5.
End of life (C1-C4)
Name Value Unit
Collected as mixed construction
1 kg
waste
Incineration 1 kg
6 Environmental Product Declaration DBC, EFCC, FEICA, IVK – Silicone-based products, group 1
5. LCA: Results
Disclaimer:
EP-freshwater: This indicator has been calculated as “kg P eq” as required in the characterization model
(EUTREND model, Struijs et al., 2009b, as implemented in ReCiPe;
http://eplca.jrc.ec.europa.eu/LCDN/developerEF.xhtml).
DESCRIPTION OF THE SYSTEM BOUNDARY (X = INCLUDED IN LCA; ND = MODULE OR INDICATOR NOT
DECLARED; MNR = MODULE NOT RELEVANT)
BENEFITS AND
CONSTRUCTI LOADS
PRODUCT STAGE ON PROCESS USE STAGE END OF LIFE STAGE BEYOND THE
STAGE SYSTEM
BOUNDARIES
7 Environmental Product Declaration DBC, EFCC, FEICA, IVK – Silicone-based products, group 1
lairetam
waR
ylppus tropsnarT
gnirutcafunaM
eht
morf
tropsnarT
etis
eht
ot
etag
ylbmessA esU
ecnanetniaM
riapeR
tnemecalpeR tnemhsibrufeR
ygrene
lanoitarepO esu
retaw
lanoitarepO esu
noitcurtsnoc-eD
noitilomed tropsnarT
gnissecorp
etsaW
lasopsiD -esueR -yrevoceR -gnilcyceR laitnetop
A1 A2 A3 A4 A5 B1 B2 B3 B4 B5 B6 B7 C1 C2 C3 C4 D
X X X X X ND ND MNR MNR MNR ND ND X X X ND X
RESULTS OF THE LCA - ENVIRONMENTAL IMPACT according to EN 15804+A2: 1 kg of silicone-based
product, group 1
Core Indicator Unit A1-A3 A4 A5 C1 C2 C3 D
GWP-total [kg CO2-Eq.] 5.31E+0 5.87E-2 6.76E-1 2.79E-4 1.24E-2 9.45E-1 -6.25E-1
GWP-fossil [kg CO2-Eq.] 5.36E+0 5.81E-2 5.61E-1 2.66E-4 1.18E-2 4.29E-1 -6.23E-1
GWP-biogenic [kg CO2-Eq.] -5.89E-2 1.70E-4 1.15E-1 1.24E-5 5.42E-4 5.15E-1 -1.43E-3
GWP-luluc [kg CO2-Eq.] 5.28E-3 4.70E-4 5.72E-5 6.39E-9 2.79E-7 3.50E-5 -4.11E-4
ODP [kg CFC11-Eq.] 1.99E-13 6.98E-18 2.04E-15 2.84E-20 1.24E-18 3.02E-16 -6.11E-15
AP [mol H+-Eq.] 1.61E-2 1.74E-4 2.36E-4 3.60E-6 3.73E-5 5.25E-4 -8.45E-4
EP-freshwater [kg P-Eq.] 9.35E-6 1.77E-7 1.02E-7 5.75E-11 2.51E-9 1.04E-7 -7.56E-7
EP-marine [kg N-Eq.] 3.60E-3 7.75E-5 5.49E-5 1.63E-6 1.72E-5 2.01E-4 -2.21E-4
EP-terrestrial [mol N-Eq.] 3.92E-2 8.68E-4 7.40E-4 1.79E-5 1.89E-4 2.52E-3 -2.37E-3
POCP [kg NMVOC-Eq.] 1.43E-2 1.53E-4 9.64E-3 4.91E-6 3.39E-5 5.22E-4 -6.38E-4
ADPE [kg Sb-Eq.] 1.09E-4 4.16E-9 1.09E-6 8.06E-12 3.52E-10 4.62E-9 -9.80E-8
ADPF [MJ] 9.79E+1 7.73E-1 1.07E+0 3.81E-3 1.66E-1 5.52E-1 -1.06E+1
[m³ world-Eq
WDP 1.67E+0 5.19E-4 7.65E-2 5.27E-7 2.30E-5 1.57E-1 -6.07E-2
deprived]
GWP = Global warming potential; ODP = Depletion potential of the stratospheric ozone layer; AP = Acidification potential of land and water; EP =
Caption Eutrophication potential; POCP = Formation potential of tropospheric ozone photochemical oxidants; ADPE = Abiotic depletion potential for non-
fossil resources; ADPF = Abiotic depletion potential for fossil resources; WDP = Water (user) deprivation potential
RESULTS OF THE LCA - INDICATORS TO DESCRIBE RESOURCE USE according to EN 15804+A2: 1 kg of
silicone-based product, group 1
Indicator Unit A1-A3 A4 A5 C1 C2 C3 D
PERE [MJ] 3.77E+1 4.35E-2 1.31E+0 1.20E-5 5.25E-4 9.36E-2 -2.17E+0
PERM [MJ] 9.05E-1 0.00E+0 -9.05E-1 0.00E+0 0.00E+0 0.00E+0 0.00E+0
PERT [MJ] 3.86E+1 4.35E-2 4.03E-1 1.20E-5 5.25E-4 9.36E-2 -2.17E+0
PENRE [MJ] 8.11E+1 7.74E-1 8.43E+0 3.81E-3 1.67E-1 1.00E+1 -1.06E+1
PENRM [MJ] 1.68E+1 0.00E+0 -7.36E+0 0.00E+0 0.00E+0 -9.45E+0 0.00E+0
PENRT [MJ] 9.79E+1 7.74E-1 1.07E+0 3.81E-3 1.67E-1 5.52E-1 -1.06E+1
SM [kg] 0.00E+0 0.00E+0 0.00E+0 0.00E+0 0.00E+0 0.00E+0 0.00E+0
RSF [MJ] 0.00E+0 0.00E+0 0.00E+0 0.00E+0 0.00E+0 0.00E+0 0.00E+0
NRSF [MJ] 0.00E+0 0.00E+0 0.00E+0 0.00E+0 0.00E+0 0.00E+0 0.00E+0
FW [m³] 5.18E-2 5.03E-5 1.92E-3 2.16E-8 9.41E-7 3.70E-3 -2.51E-3
PERE = Use of renewable primary energy excluding renewable primary energy resources used as raw materials; PERM = Use of
renewable primary energy resources used as raw materials; PERT = Total use of renewable primary energy resources; PENRE = Use of
non-renewable primary energy excluding non-renewable primary energy resources used as raw materials; PENRM = Use of non-
Caption
renewable primary energy resources used as raw materials; PENRT = Total use of non-renewable primary energy resources; SM = Use
of secondary material; RSF = Use of renewable secondary fuels; NRSF = Use of non-renewable secondary fuels; FW = Use of net fresh
water
RESULTS OF THE LCA – WASTE CATEGORIES AND OUTPUT FLOWS according to EN 15804+A2:
1 kg of silicone-based product, group 1
Indicator Unit A1-A3 A4 A5 C1 C2 C3 D
HWD [kg] 7.39E-7 3.60E-8 7.47E-9 3.70E-13 1.62E-11 1.77E-9 -4.20E-9
NHWD [kg] 1.27E+0 1.18E-4 1.74E-2 3.90E-7 1.70E-5 1.36E-1 -4.73E-3
RWD [kg] 3.96E-3 9.58E-7 4.49E-5 4.09E-9 1.79E-7 2.51E-5 -7.40E-4
CRU [kg] 0.00E+0 0.00E+0 0.00E+0 0.00E+0 0.00E+0 0.00E+0 0.00E+0
MFR [kg] 0.00E+0 0.00E+0 0.00E+0 0.00E+0 0.00E+0 0.00E+0 0.00E+0
MER [kg] 0.00E+0 0.00E+0 0.00E+0 0.00E+0 0.00E+0 0.00E+0 0.00E+0
EEE [MJ] 0.00E+0 0.00E+0 1.24E+0 0.00E+0 0.00E+0 0.00E+0 0.00E+0
EET [MJ] 0.00E+0 0.00E+0 2.22E+0 0.00E+0 0.00E+0 0.00E+0 0.00E+0
Caption HWD = Hazardous waste disposed; NHWD = Non-hazardous waste disposed; RWD = Radioactive waste disposed; CRU = Components
for re-use; MFR = Materials for recycling; MER = Materials for energy recovery; EEE = Exported electrical energy; EEE = Exported
thermal energy
RESULTS OF THE LCA – additional impact categories according to EN 15804+A2-optional:
1 kg of silicone-based product, group 1
Indicator Unit A1-A3 A4 A5 C1 C2 C3 D
[Disease
PM ND ND ND ND ND ND ND
Incidence]
[kBq U235-
IRP ND ND ND ND ND ND ND
Eq.]
ETP-fw [CTUe] ND ND ND ND ND ND ND
HTP-c [CTUh] ND ND ND ND ND ND ND
HTP-nc [CTUh] ND ND ND ND ND ND ND
SQP [-] ND ND ND ND ND ND ND
PM = Potential incidence of disease due to PM emissions; IR = Potential Human exposure efficiency relative to U235; ETP-fw = Potential
Caption comparative Toxic Unit for ecosystems; HTP-c = Potential comparative Toxic Unit for humans (cancerogenic); HTP-nc = Potential
comparative Toxic Unit for humans (not cancerogenic); SQP = Potential soil quality index
Potential Human exposure efficiency relative to U235, Disclaimer 1 – This impact category deals mainly with the
eventual impact of low dose ionizing radiation on human health of the nuclear fuel cycle. It does not consider
effects due to possible nuclear accidents, occupational exposure or radioactive waste disposal in underground
facilities. Potential ionizing radiation from the soil, radon and (from) some construction materials is also not
measured by this indicator.
ADP minerals & metals, ADP fossil, WDP, ETF-fw, HTP-c, HTP-nc, SQP, Disclaimer 2 – The results of this
environmental impact indicator shall be used with care as the uncertainties on these results are high or as there is
limited experience with the indicator.
Additional environmental impact indicators (suggested by EN15804, table 4) are not declared in the EPD. The
results of this environmental impact indicator shall be used with care as the uncertainties on these results are high
and as there is limited experience with the indicator (see ILCD classification in EN 15804, table 5). For this
reason, results based on these indicators are not considered suitable for a decision-making process and are thus
not declared in the EPD.
6. LCA: Interpretation
The majority of impacts are associated with the that Primary Energy Demand – Renewable (PERT)
production phase (A1-A3). The most significant generally represents a small percentage of the
contribution to the production phase impacts is the production phase primary energy demand with the bulk
upstream production of raw materials as a main driver. of the demand coming from non-renewable energy
Another contributor in the production phase, in the resources.
category of Photochemical ozone formation (POCP), is Transportation to the construction site (A4) and the
the plastic used as a packaging material. Emissions installation process (A5) make a low contribution to the
associated with the manufacturing of products also overall impacts. Climate change from land use change
have a high influence on Ozone Depletion Potential is the only indicator influenced by transport processes,
(ODP) in the production phase. In all EPDs, CO is the due to the diesel production used as fuel, because part
2
most important contributor to Global Warming Potential of this diesel has been produced from bio-based raw
(GWP). For the Acidification Potential (AP), NOx and materials.
SO contribute the largest share. The installation phase influence mainly Photochemical
2
The majority of life cycle energy consumption takes ozone formation indicator, due to the emission of VOC
place during the production phase (A1-A3). Significant during the operations. These emissions are not only
contributions to Primary Energy Demand – Non- directly related to the pre-products in the resins, but
renewable (PENRT) come from the energy resources they are related to the reaction products between pre-
used in the production of raw materials. The largest products and air components (water and oxygen).
contributor to Primary Energy Demand – Renewable The end-of-life phases influence climate change
(PERT) impacts comes from the consumption of indicators, due to the thermal treatment process of the
renewable energy resources required for the silicon-based products occurring in the C3 module.
generation and supply of electricity. It should be noted
7. Requisite evidence
VOC Evidence pertaining to VOC emissions shall show
Special tests and evidence have not been carried out - either an attestation of compliance with,
or provided within the framework of drawing up this - or documentation of test data that are required in
Model EPD. Some member states require special any of the existing regulations or in any of the existing
documentation on VOC emissions into indoor air for voluntary labelling programs for low-emitting products,
specific areas of application. This documentation, as as far as these
well as documentation for voluntary VOC labelling, has (1) include limits for the parameters TVOC, TSVOC,
to be provided separately and is specific to the product carcinogens, formaldehyde, acetaldehyde, LCI limits
in question. for individual substances (including but not limited to
8 Environmental Product Declaration DBC, EFCC, FEICA, IVK – Silicone-based products, group 1
the European list of harmonized LCIs), and the R- Examples for the applied limits after 28 days of storage
value; in a ventilated test chamber are:
(2) base their test methods on EN 16516; - TVOC: 1000 µg/m³
(3) perform testing and apply the limits after 28 days - TSVOC: 100 µg/m³
of storage in a ventilated test chamber, under the - Each carcinogen: 1 µg/m³
conditions specified in EN 16516; some regulations - Formaldehyde: 100 µg/m³
and programs also have limits after 3 days, on top of - LCI: different per substance involved
the 28 days limits; - R-value: 1 (meaning that, in total, 100 % of the
(4) express the test results as air concentrations in combined LCI values must not be exceeded).
the European Reference Room, as specified in EN Informative Annexes (2 tables):
16516. Table 1 shown below is an overview of the most
relevant regulations and specifications as of October
Examples of such regulations are the Belgian Royal 2021, as regards requirements after 3 days of storage
Decree C-2014/24239, or the German AgBB/ ABG. in a ventilated test chamber.
Examples of such voluntary labelling programs are Table 2 provides an overview of the most relevant
EMICODE, Blue Angel or Indoor Air Comfort. regulations and specifications as of October 2021, as
regards requirements after 28 days of storage in a
Relevant test results shall be produced either by an ventilated test chamber. Some details may be missing
ISO 17025 accredited commercial test lab or by a in the table due to lack of space. Values given
qualified internal test lab of the manufacturer. represent maximum values/limits.
8. References
ETAG 002-1 Structural Sealant Glazing Kits (SSGK) – Part 1:
ETAG 002-1:2012 (used as EAD) Supported and unsupported Systems
9 Environmental Product Declaration DBC, EFCC, FEICA, IVK – Silicone-based products, group 1
EN 15804
RAL UZ 123 EN 15804+A2:2019+AC:2021, Sustainability of
RAL UZ 123:2019 Basis for awarding the "Low- construction works — Environmental Product
emission sealants for interiors" environmental Declarations — Core rules for the product category of
certificate construction products.
EN ISO 7389 EN 16516
EN ISO 7389:2003 Building construction – Jointing EN 16516:2017
products – Determination of elastic recovery of Construction products - Assessment of release of
sealants dangerous substances - Determination of emissions
into indoor air
EN ISO 7390
EN ISO 7390:2003 Building construction – Jointing EN ISO 17025
products – Determination of resistance to flow of EN ISO 17025: 2018-03
sealants General requirements for the competence of testing
and calibration laboratories
EN ISO 8339
EN ISO 8339: 2005 Building construction – Sealants – 2000/532/EC
Determination of tensile properties (Extension to Commission decision dated 3 May 2000 replacing
break) decision 94/3/EC on a waste directory in accordance
with Article 1 a) of Council Directive 75/442/EEC on
EN 10563 waste and Council decision 94/904/EC on a directory
EN ISO 10563:2017 Building construction – Sealants – of hazardous waste in terms of Article 1, paragraph 4
Determination of change in mass and volume of Directive 91/689/EEC on hazardous waste
EN ISO 10590 Belgian Royal Decree C-2014/24239
EN ISO 10590:2005 Building construction – Sealants – Belgisch Staatsblad 8 MEI 2014, p. 60603. —
Determination of tensile properties of sealants at Koninklijk besluit tot vaststelling van de
maintained extension after immersion in water drempelniveaus voor de emissies naar het
binnenmilieu van bouwproducten voor bepaalde
EN ISO 10591 geoogde gebruiken
EN ISO 10591:2005 Building construction – Sealants -
Determination of adhesion/cohesion properties of Blue Angel
sealants after immersion in water Environmental label organised by the federal
government of Germany www.blauer-engel.de
EN ISO 11431
EN ISO 11431:2002 Building construction – Jointing Candidate list
products – Determination of adhesion/cohesion Candidate List of substances of very high concern for
properties of sealants after exposure to heat, water Authorisation, published in accordance with Article
and artificial light through glass 59(10) of the REACH Regulation, ECHA,
www.echa.europa.eu/candidate-list-table
EN 13501-1
EN 13501-1:2018 Fire classification of construction CPR
products and building elements – Part 1: Classification CPR Regulation (EU) No 305/2011 of the European
using data from reaction to fire tests Parliament and of the Council of 9 March 2011 laying
down harmonised conditions for the marketing of
ISO 14025 construction products and repealing Council Directive
DIN EN ISO 14025:2011-10, Environmental labels and 89/106/EEC
declarations — Type III environmental declarations —
Principles and procedures Decopaint Directive
Directive 2004/42/CE of the European Parliament and
EN 15651-1 the council of 21 April 2004 on the limitation of
EN 15651-1:2012 Sealants for non-structural use in emissions of volatile organic compounds due to the
joints in buildings and pedestrian walkways – Part 1: use of organic solvents in certain paints and varnishes
Sealants for façade elements and vehicle refinishing products and amending
Directive 1999/13/EC
EN 15651-2
EN 15651-2:2012 Sealants for non-structural use in EMICODE
joints in buildings and pedestrian walkways– Part 2: EMICODE, GEV – Gemeinschaft
Sealants for glazing Emissionskontrollierte Verlegewerkstoffe, Klebstoffe
und Bauprodukte e. V. (pub.).www.emicode.de
EN 15651-3
EN 15651-3:2012 Sealants for non-structural use in GaBi 10
joints in buildings and pedestrian walkways – Part 3: GaBi 10: Software and database for comprehensive
Sealants for sanitary joints analysis. LBP, University of Stuttgart and Sphera, 2020
EN 15651-4 GaBi 10 documentation
EN 15651-4:2012 Sealants for non-structural use in Gabi 10: documentation of GaBi 10 data sets from the
joints in buildings and pedestrian walkways – Part 4: data base for Life Cycle Engineering LBP, University of
Sealants for pedestrian walkways Stuttgart and Sphera, http://documentation.gabi-
software.com/, 2020
10 Environmental Product Declaration DBC, EFCC, FEICA, IVK – Silicone-based products, group 1
report, Version 1.1, Institut Bauen und Umwelt e.V.,
German AgBB 2021-01
Committee for Health-related Evaluation of Building
Products: health-related evaluation of emissions of PCR Part B
volatile organic compounds (VOC and SVOC) from Product Category Rules for Construction Products,
building products; status: June 2012 Part B: Building sealants, 2019-04
www.umweltbundesamt.de/produkte/bauprodukte/agb
b.htm REACH
Directive (EG) No. 1907/2006 of the European
IBU 2021 Parliament and of the Council dated 18 December
Institut Bauen und Umwelt e.V.: General Instructions 2006 on the registration, evaluation, approval and
for the EPD programme of Institut Bauen und Umwelt restriction of chemical substances (REACH), for
e.V. EPD programme. Version 2.0. Berlin: Institut establishing a European Agency for chemical
Bauen und Umwelt e.V., 2021 substances, for amending Directive 1999/45/EC and
www.ibu-epd.com for annulment of Directive (EEC) No. 793/93 of the
Council, Directive (EC) No. 1488/94 of the
Indoor Air Comfort Commission, Guideline 76/769/EEC of the Council and
Product certification by Eurofins, Hamburg, Germany Guidelines 91/155/EEC, 93/67/EEC, 93/105/EC and
www.eurofins.com 2000/21/EC of the Commission.
PCR Part A
Product Category Rules for Building-Related Products
and Services, Part A: Calculation Rules for the Life
Cycle Assessment and Requirements on the Project
11 Environmental Product Declaration DBC, EFCC, FEICA, IVK – Silicone-based products, group 1
Publisher
Institut Bauen und Umwelt e.V. Tel +49 (0)30 3087748- 0
Panoramastr. 1 Fax +49 (0)30 3087748- 29
10178 Berlin Mail info@ibu-epd.com
Germany Web www.ibu-epd.com
Programme holder
Institut Bauen und Umwelt e.V. Tel +49 (0)30 - 3087748- 0
Panoramastr 1 Fax +49 (0)30 – 3087748 - 29
10178 Berlin Mail info@ibu-epd.com
Germany Web www.ibu-epd.com
Author of the Life Cycle
Assessment Tel +49 711 341817-0
Sphera Solutions GmbH Fax +49 711 341817-25
Hauptstraße 111- 113 Mail info@sphera.com
70771 Leinfelden-Echterdingen Web www.sphera.com
Germany
Owner of the Declaration
Industrieverband Klebstoffe e.V Tel +49 (0)211 67931-10
Völklinger Straße 4 Fax +49 (0)211 67931-33
40219 Düsseldorf Mail info@klebstoffe.com
Germany Web www.klebstoffe.com
FEICA - Association of the Tel +32 (0)267 673 20
European Adhesive and Sealant Fax +32 (0)267 673 99
Industry Mail info@feica.eu
Rue Belliard 40 box 10 Web www.feica.eu
1040 Brussels
Belgium
Tel +32289720-39
Fax +32289720-37
EFCC - European Federation for Mail info@efcc.be
Construction Chemicals Web www.efcc.eu
Boulevard du Triomphe 172
1160 Brussels
Belgium
Tel +49 (0)69 2556-1318
Fax +49 (0)69 2556-1319
Mail info@deutsche-bauchemie.de
Deutsche Bauchemie e.V. Web www.deutsche-bauchemie.de
Mainzer Landstr. 55
60329 Frankfurt
Germany
