ENVIRONMENTAL PRODUCT DECLARATION
as per ISO 14025 and EN 15804+A1
Owner of the Declaration Balsan
Programme holder Institut Bauen und Umwelt e.V. (IBU)
Publisher Institut Bauen und Umwelt e.V. (IBU)
Declaration number EPD-BAL-20210254-CCA1-EN
Issue date 27.10.2021
Valid to 26.10.2026
NEXUS / NEXUS LINK
tufted carpet tiles made of recycled pile material
BALSAN
www.ibu-epd.com | https://epd-online.com
Umwelt Produktdeklaration Name des Herstellers – Name des Produkts
General Information
Balsan NEXUS / NEXUS LINK - tufted carpet
tiles made of recycled pile material
Programme holder Owner of the declaration
IBU – Institut Bauen und Umwelt e.V. Balsan
Panoramastr. 1 Corbilly - D14
10178 Berlin 36330 Arthon
Germany France
Declaration number Declared product / declared unit
EPD-BAL-20210254-CCA1-EN 1 m² tufted carpet tiles NEXUS.
This declaration is based on the product Scope:
category rules: The manufacturer declaration applies to the tufted
Floor coverings, 02/2018 carpet tiles NEXUS / NEXUS LINK with the GUT-
(PCR checked and approved by the SVR) PRODIS license number FE54F11B.
The products are produced in the Balsan
Issue date manufacturing sites Arthon (tufting and precoating) and
Neuvy-Saint-Sépulchre (back coating), France.
27.10.2021
The declaration is only valid in conjunction with a valid
GUT-PRODIS license of the product.
Valid to
26.10.2026
The owner of the declaration shall be liable for the
underlying information and evidence; the IBU shall not
be liable with respect to manufacturer information, life
cycle assessment data and evidences.
The EPD was created according to the specifications
of EN 15804+A1. In the following, the standard will be
simplified as EN 15804.
Verification
The standard EN 15804 serves as the core PCR
Independent verification of the declaration and data
according to ISO 14025:2010
Dipl. Ing. Hans Peters internally x externally
(chairman of Institut Bauen und Umwelt e.V.)
Dr. Alexander Röder Angela Schindler
(Managing Director Institut Bauen und Umwelt e.V.)) (Independent verifier)
Product
Product description/Product definition For the application and use of the product the
NEXUS / NEXUS LINK - tufted carpet tiles having a respective national provisions apply.
surface pile of solution-dyed polyamide 6 with 100%
recycled content, a polyester primary backing with Application
100% recycled content and a bitumen based heavy According to the use class as defined in EN 1307 the
backing with a fibre glass reinforcement and a products can be used in all professional areas which
polyester covering fleece. require class 33 or less.
The recycled content amounts to 20%.
For the placing on the market of the product in the
European Union/European Free Trade Association
(EU/EFTA) (with the exception of Switzerland)
Regulation (EU) No. 305/2011 Construction Product
Technical Data
Regulation (CPR) applies. The product needs a
The performance data listed in the DoP apply.
Declaration of Performance (DoP) taking into
consideration EN 14041: 2018-05, Resilient, textile and
laminate floor coverings - Essential characteristics, and
the CE-marking. The DoP of the product can be found
on the manufacturer's technical information section.
2 Environmental Product Declaration Balsan – NEXUS / NEXUS LINK - tufted carpet tiles
Name Value Unit This product contains substances listed in the ECHA
Product Form Tiles 50 cm x 50 cm - candidate list (16.01.2020) or other carcinogenic,
Type of manufacture Tufted tiles - mutagenic or reprotoxic (CMR) substances in
Polyamide 6, categories 1A or 1B which are not on the candidate list
Yarn type -
100 % recycled exceeding 0.1 percentage by mass: no
Coloration Solution dyed yarn The products are registered in the GUT-PRODIS
Primary backing Polyester, 100% recycled Information System. The PRODIS system ensures the
Bitumen based heavy compliance with limitations of various chemicals and
Secondary backing backing - Volatile Organic Compound (VOC)-emissions and a
Total pile weight 850 g/m² ban on the use of all substances that are listed as
'Substances of Very High Concern' (SVHC) under
Surface pile weight 470 g/m2
REACH.
Total carpet weight 5000 g/m2
Total thickness 7.9 mm
Reference service life
A calculation of the reference service life according to
ISO 15686 is not possible.
Performance data of the product in accordance with
The service life of textile floor coverings strongly
the declaration of performance with respect to its
depends on the correct installation taking into account
essential characteristics according to EN 14041: 2018-
the declared use classification and the adherence to
05, Resilient, textile and laminate floor coverings -
cleaning and maintenance instructions.
Essential characteristics. Additional product properties
A minimum service life of 10 years can be
in accordance with EN 1307 can be found on the
assumed, technical service life can be considerably
Product Information System PRODIS using the
longer.
PRODIS registration number of the product (www.pro-
dis.info) or on the manufacturer's technical information
section (www.balsan.com).
Base materials/Ancillary materials
Name Value Unit
Polyamide 6 17.0 %
Polyester 4.5 %
SBR-latex 3.5 %
Mineral filler 53.1 %
Aluminum hydroxide 5.2 %
Bitumen 15.9 %
Glass fibre 0.7 %
Additives 0.1 %
LCA: Calculation rules
Declared Unit residual waste (except radioactive waste). Benefits for
generated electricity and steam due to the incineration
of production waste are aggregated.
Name Value Unit Biogenic carbon that is stored in renewable material
Declared unit 1 m2 (packaging paper) is taken into account as well as the
Grammage 5 kg/m2 associated carbon dioxide uptake from the air from
Gross density 633 kg/m3 which this biogenic carbon comes.
The declared unit refers to 1 m2 produced textile floor
covering. The output of module A5 'Assembly' is 1 m2 A4 Transport:
installed textile floor covering. Transport of the packed textile floor covering
from factory gate to the place of installation.
System boundary A5 Installation:
Installation of the textile floor covering, processing of
Type of EPD: Cradle-to-grave installation waste and packaging waste up to the
landfill disposal of residual waste (except radioactive
System boundaries of modules A, B, C, D: waste), the production of the amount of carpet that
Modules C3, C4 and D are indicated separately for occurs as installation waste including its transport to
three end-of-life scenarios: the place of installation.
1 - landfill disposal Generated electricity and steam due to the incineration
2 - municipal waste incineration of waste are listed in the result table as exported
3 - recovery in a cement plant energy.
Biogenic carbon that is stored in renewable materials
A1-A3 Production: in packaging paper is released as carbon dioxide
Energy supply and production of the basic material, emissions into the air at the end of life in module A5.
processing of secondary material, auxiliary material, Preparation of the floor and auxiliary materials
transport of the material to the manufacturing site, (adhesives, fixing agents, PET connectors) are beyond
emissions, waste water treatment, packaging material the system boundaries and not taken into account.
and waste processing up to the landfill disposal of
3 Environmental Product Declaration Balsan – NEXUS / NEXUS LINK - tufted carpet tiles
B1 Use: transport to the cement plant, emissions from the
Indoor emissions during the use stage. After the first incineration. The biogenic carbon that is stored in the
year, no product-related Volatile Organic Compound renewable materials of the floor covering is released
(VOC) emissions are relevant due to known VOC into the air as carbon dioxide emissions.
decay curves of the product.
C4 Disposal
B2 Maintenance: C4-1: Impact from landfill disposal,
Cleaning of the textile floor covering for a period of 1 C4-2: The carpet waste leaves the system in
year: module C3-2,
Vacuum cleaning – electricity supply C4-3: The pre-processed carpet waste leaves the
Wet cleaning – electricity, water consumption, system in module C3-3.
production of the cleaning agent, waste water
treatment. D Recycling potential:
The declared values in this module have to be Calculated benefits result from materials exclusive
multiplied by the assumed service life of the floor secondary materials (net materials).
covering in the building in question. D-A5: Benefits for generated energy due
to incineration of packaging and installation waste
B3 - B7: (incineration plant with R1 > 0.6),
The modules are not relevant and therefore not D-1: Benefits for generated energy due to landfill
declared. disposal of carpet waste at the end-of-life,
D-2: Benefits for generated energy due to incineration
C1 De-construction: of carpet waste at the end-of-life (incineration plant
The floor covering is de-constructed manually and no with R1 > 0.6),
additional environmental impact is caused. D-3: Benefits for saved fossil energy and saved
inorganic material due to recovery of the carpet in a
C2 Transport: cement plant.
Transport of the carpet waste to a landfill, to the
municipal waste incineration plant (MWI) or to the Comparability
waste collection facility for recycling. Basically, a comparison or an evaluation of EPD data
is only possible if all the data sets to be compared
C3 Waste processing: were created according to EN 15804 and the building
C3-1: Landfill disposal needs no waste processing. context, respectively the product-specific
C3-2: Impact from waste incineration (plant with characteristics of performance, are taken into account.
R1>0.6), generated electricity and steam are listed in
the result table as exported energy. Background data are taken from the GaBi database
C3-3: Collection of the carpet waste for recovery in the 2021. Remaining data gaps are covered by the
cement industry, waste processing (granulating), ecoinvent 3.7 database
LCA: Scenarios and additional technical information
The following information refer to the declared modules calculated in order to obtain the overall environmental
and are the basis for calculations or can be used for impacts.
further calculations. Name Value Unit
Maintenance cycle (wet cleaning) 1.5 1/year
Transport to the construction site (A4) Maintenance cycle (vacuum cleaning) 208 1/year
Name Value Unit Water consumption (wet cleaning) 0.004 m3
Litres of fuel (truck, EURO 0-6 mix) 0.012 l/100km Cleaning agent (wet cleaning) 0.09 kg
Transport distance 700 km Electricity consumption 0.314 kWh
Capacity utilisation (including empty Further information on cleaning and maintenance see
55 %
runs) www.balsan.com
Gross density of products transported 633 kg/m3
End of Life (C1-C4)
Installation in the building (A5) Three different end-of-life scenarios are declared and
Name Value Unit the results are indicated separately in module C.
Material loss 0.15 kg Each scenario is calculated as a 100% scenario.
Polyethylene packaging waste and installation waste
are considered to be incinerated in a municipal waste Scenario 1: 100% landfill disposal
incineration plant. Cardboard is going to be recycled. Scenario 2: 100% municipal waste incineration (MWI)
Preparation of the floor and auxiliaries (adhesives, with R1>0.6
fixing agents, PET connectors etc.) are not taken into Scenario 3: 100% recycling in the cement industry
account.
Maintenance (B2)
The values for cleaning refer to 1 m2 floor covering
used in commercial areas per year. Depending on the
application based on ISO 10874, the technical service
life recommended by the manufacturer and the If combinations of these scenarios have to be
anticipated strain on the floor by customers, the case- calculated this should be done according to the
specific useful life can be established. Based on this following scheme:
useful life the effects of Module B2 need to be EOL-impact = x% impact (Scenario 1)
4 Environmental Product Declaration Balsan – NEXUS / NEXUS LINK - tufted carpet tiles
+ y% impact (Scenario 2)
+ z% impact (Scenario 3)
with x% + y% + z% = 100%
Name Value Unit
Collected as mixed construction waste
5 kg
(scenario 1 and 2)
Collected separately (scenario 3) 5 kg
Landfilling (scenario 1) 5 kg
Energy recovery (scenario 2) 5 kg
Energy recovery (scenario 3) 2.05 kg
Recycling (scenario 3) 2.95 kg
Reuse, recovery and/or recycling potentials (D),
relevant scenario information
Recovery or recycling potentials due to the three end-
of-life scenarios (module C) are indicated separately.
Recycling in the cement industry (scenario 3)
VDZ e.V.
The organic material of the carpet is used as
secondary fuel in a cement kiln. It mainly substitutes
for lignite (65.5%), hard coal (26.2%) and petrol coke
(8.6%).
The inorganic material is substantially integrated into
the cement clinker and substitutes for original material
input.
5 Environmental Product Declaration Balsan – NEXUS / NEXUS LINK - tufted carpet tiles
LCA: Results
The declared result figures in module B2 have to be multiplied by the assumed service life (in years) of the floor
covering in the building under consideration.
Information on non-relevant modules: Modules B3 - B7 are not relevant during the service life of the carpet.
Modules C1, C3/1, C4/2 and C4/3 cause no additional impact (see chapter "LCA: Calculation rules" in this
document). All these modules are declared and marked as 'modules not relevant/declared'. Module C2 represents
the transport for scenarios 1, 2 and 3. Column D represents module D/A5.
The calculations are based on the CML characterization factors (version August 2016).
DESCRIPTION OF THE SYSTEM BOUNDARY (X = INCLUDED IN LCA; MND = MODULE NOT DECLARED;
MNR = MODULE NOT RELEVANT)
BENEFITS AND
CONSTRUCTI LOADS
PRODUCT STAGE ON PROCESS USE STAGE END OF LIFE STAGE BEYOND THE
STAGE SYSTEM
BOUNDARIES
6 Environmental Product Declaration Balsan – NEXUS / NEXUS LINK - tufted carpet tiles
lairetam
waR
ylppus tropsnarT
gnirutcafunaM
eht
morf
tropsnarT
etis
eht
ot
etag
ylbmessA esU
ecnanetniaM
riapeR
tnemecalpeR tnemhsibrufeR
ygrene
lanoitarepO esu
retaw
lanoitarepO esu
noitcurtsnoc-eD
noitilomed tropsnarT
gnissecorp
etsaW
lasopsiD -esueR -yrevoceR -gnilcyceR laitnetop
A1 A2 A3 A4 A5 B1 B2 B3 B4 B5 B6 B7 C1 C2 C3 C4 D
X X X X X X X MNR MNR MNR MND MND MND X X X X
RESULTS OF THE LCA - ENVIRONMENTAL IMPACT according to EN 15804+A1: 1 m² floorcovering
Parameter Unit A1-A3 A4 A5 B1 B2 C2 C3/2 C3/3 C4/1 D D/1 D/2 D/3
GWP [kg CO2-Eq.] 4.20E+0 2.96E-1 4.46E-1 0.00E+0 2.92E-1 1.66E-2 5.34E+0 5.41E+0 3.40E-1 -1.34E-2 0.00E+0 -3.96E-1 -3.02E-1
-1.88E- -5.48E- -1.80E-
ODP [kg CFC11-Eq.] 9.57E-9 5.16E-172.87E-100.00E+0 1.08E-8 2.90E-182.36E-153.25E-151.15E-15 0.00E+0
16 15 15
AP [kg SO2-Eq.] 1.32E-2 1.22E-3 5.32E-4 0.00E+0 1.08E-3 6.86E-5 3.21E-3 3.43E-3 8.81E-4 -1.47E-5 0.00E+0 -4.32E-4 -9.87E-4
EP [kg (PO4)3--Eq.] 2.51E-3 3.12E-4 1.09E-4 0.00E+0 3.02E-4 1.75E-5 7.85E-4 8.35E-4 9.56E-4 -2.06E-6 0.00E+0 -6.06E-5 -1.48E-4
POCP [kg ethene-Eq.] 9.26E-4 -5.24E-4 1.69E-5 6.29E-5 1.45E-4 -2.94E-5 1.99E-4 1.29E-4 7.93E-5 -1.39E-6 0.00E+0 -4.09E-5 -1.03E-4
ADPE [kg Sb-Eq.] 4.88E-6 2.62E-8 1.54E-7 0.00E+0 2.74E-6 1.47E-9 2.21E-7 2.34E-7 6.52E-8 -2.37E-9 0.00E+0 -6.92E-8 -1.59E-7
ADPF [MJ] 9.80E+1 4.03E+0 3.17E+0 0.00E+0 6.76E+0 2.26E-1 3.21E+0 4.08E+0 5.07E+0 -1.96E-1 0.00E+0-5.80E+0-3.34E+1
GWP = Global warming potential; ODP = Depletion potential of the stratospheric ozone layer; AP = Acidification potential of land and water; EP =
Caption Eutrophication potential; POCP = Formation potential of tropospheric ozone photochemical oxidants; ADPE = Abiotic depletion potential for non-
fossil resources; ADPF = Abiotic depletion potential for fossil resources
RESULTS OF THE LCA - INDICATORS TO DESCRIBE RESOURCE USE according to EN 15804+A1: 1 m²
floorcovering
Parameter Unit A1-A3 A4 A5 B1 B2 C2 C3/2 C3/3 C4/1 D D/1 D/2 D/3
PERE [MJ] 4.67E+1 2.25E-1 2.85E+0 0.00E+0 1.23E+0 1.26E-2 5.59E-1 8.17E-1 3.79E-1 -4.85E-2 0.00E+0 -1.41E+0 -4.26E-1
PERM [MJ] 1.38E+0 0.00E+0 -1.38E+0 0.00E+0 0.00E+0 0.00E+0 0.00E+0 0.00E+0 0.00E+0 0.00E+0 0.00E+0 0.00E+0 0.00E+0
PERT [MJ] 4.81E+1 2.25E-1 1.47E+0 0.00E+0 1.23E+0 1.26E-2 5.59E-1 8.17E-1 3.79E-1 -4.85E-2 0.00E+0 -1.41E+0 -4.26E-1
PENRE [MJ] 6.63E+1 4.04E+0 3.36E+0 0.00E+0 7.85E+0 2.27E-1 3.97E+1 4.08E+1 5.23E+0 -2.35E-1 0.00E+0 -6.94E+0 -3.36E+1
PENRM [MJ] 3.63E+1 0.00E+0 -4.30E-2 0.00E+0 0.00E+0 0.00E+0 -3.62E+1 -3.62E+1 0.00E+0 0.00E+0 0.00E+0 0.00E+0 0.00E+0
PENRT [MJ] 1.03E+2 4.04E+0 3.31E+0 0.00E+0 7.85E+0 2.27E-1 3.53E+0 4.59E+0 5.23E+0 -2.35E-1 0.00E+0 -6.94E+0 -3.36E+1
SM [kg] 1.13E+0 0.00E+0 3.39E-2 0.00E+0 0.00E+0 0.00E+0 0.00E+0 0.00E+0 0.00E+0 0.00E+0 0.00E+0 0.00E+0 1.69E+0
RSF [MJ] 0.00E+0 0.00E+0 0.00E+0 0.00E+0 0.00E+0 0.00E+0 0.00E+0 0.00E+0 0.00E+0 0.00E+0 0.00E+0 0.00E+0 0.00E+0
NRSF [MJ] 0.00E+0 0.00E+0 0.00E+0 0.00E+0 0.00E+0 0.00E+0 0.00E+0 0.00E+0 0.00E+0 0.00E+0 0.00E+0 0.00E+0 0.00E+0
FW [m³] 1.32E-1 2.58E-4 4.50E-3 0.00E+0 4.13E-3 1.45E-5 1.81E-2 1.83E-2 4.82E-5 -4.74E-5 0.00E+0 -1.38E-3 -3.01E-3
PERE = Use of renewable primary energy excluding renewable primary energy resources used as raw materials; PERM = Use of
renewable primary energy resources used as raw materials; PERT = Total use of renewable primary energy resources; PENRE = Use of
non-renewable primary energy excluding non-renewable primary energy resources used as raw materials; PENRM = Use of non-
Caption
renewable primary energy resources used as raw materials; PENRT = Total use of non-renewable primary energy resources; SM = Use
of secondary material; RSF = Use of renewable secondary fuels; NRSF = Use of non-renewable secondary fuels; FW = Use of net fresh
water
RESULTS OF THE LCA – WASTE CATEGORIES AND OUTPUT FLOWS according to EN 15804+A1:
1 m² floorcovering
Parameter Unit A1-A3 A4 A5 B1 B2 C2 C3/2 C3/3 C4/1 D D/1 D/2 D/3
HWD [kg] 2.47E-3 2.04E-10 7.42E-5 0.00E+0 5.90E-10 1.14E-11 6.59E-10 8.18E-10 9.40E-10 -5.20E-11 0.00E+0 -1.53E-9 -3.77E-10
NHWD [kg] 5.30E-1 6.00E-4 5.99E-2 0.00E+0 5.62E-3 3.37E-5 1.47E+0 1.47E+0 4.98E+0 -1.06E-4 0.00E+0 -3.10E-3 -1.25E-1
RWD [kg] 1.77E-3 4.89E-6 5.72E-5 0.00E+0 3.32E-4 2.74E-7 1.27E-4 2.01E-4 6.07E-5 -1.56E-5 0.00E+0 -4.54E-4 -9.69E-5
CRU [kg] 0.00E+0 0.00E+0 0.00E+0 0.00E+0 0.00E+0 0.00E+0 0.00E+0 0.00E+0 0.00E+0 0.00E+0 0.00E+0 0.00E+0 0.00E+0
MFR [kg] 1.46E-2 0.00E+0 9.20E-2 0.00E+0 0.00E+0 0.00E+0 0.00E+0 1.69E+0 0.00E+0 0.00E+0 0.00E+0 0.00E+0 0.00E+0
MER [kg] 0.00E+0 0.00E+0 0.00E+0 0.00E+0 0.00E+0 0.00E+0 0.00E+0 0.00E+0 0.00E+0 0.00E+0 0.00E+0 0.00E+0 0.00E+0
EEE [MJ] 0.00E+0 0.00E+0 1.87E-1 0.00E+0 0.00E+0 0.00E+0 6.02E+0 0.00E+0 0.00E+0 0.00E+0 0.00E+0 0.00E+0 0.00E+0
EET [MJ] 0.00E+0 0.00E+0 3.54E-1 0.00E+0 0.00E+0 0.00E+0 1.14E+1 6.67E+1 0.00E+0 0.00E+0 0.00E+0 0.00E+0 0.00E+0
HWD = Hazardous waste disposed; NHWD = Non-hazardous waste disposed; RWD = Radioactive waste disposed; CRU = Components
Caption for re-use; MFR = Materials for recycling; MER = Materials for energy recovery; EEE = Exported electrical energy; EEE = Exported
thermal energy
Not all of the life cycle inventories applied in this study support the methodological approach for the waste and
water indicators. The data are based on publications of industry. The indicators for waste and water of the system
are evaluated but contain a higher degree of uncertainty.
References
EN 1307 CML characterization factors
DIN EN 1307: 2014+A1:2016+A2:2018-05: Textile Impact assessment characterization factors, version
floor coverings - Classification 4.7, August 2016, Institute of Environmental Sciences -
'Centrum voor Milieuwetenschappen in Leiden' (CML),
EN 13501-1 Leiden, The Netherlands
DIN EN 13501-1:2019-05: Fire classification of
construction products and building elements - Part 1:
Classification using data from reaction to fire tests ECHA candidate list
Candidate List of substances of very high concern
EN 14041 (SVHCs) for authorisation, 16.01.2020, European
DIN EN 14041: 2018-05: Resilient, textile and laminate Chemicals Agency (ECHA), Helsinki, Finland
floor coverings - Essential characteristics
ecoinvent 3.7
EN 15804 ecoinvent, Zurich, Switzerland, database version 3.7,
EN 15804:2012-04+A1 2013/, Sustainability of published September 2020
construction works — Environmental Product
Declarations — Core rules for the product category of GaBi database 2021
construction products GaBi Software-System and Database for Life Cycle
Engineering, thinkstep AG, Leinfelden-Echterdingen,
EN 16810 2021-2
DIN EN 16810: 2017-08: Resilient, textile and laminate
floor coverings – Environmental product declarations – IBU 2021
Product category rules IBU (2021): General Programme Instructions for the
Preparation of EPDs at the Institut Bauen und Umwelt
ISO 10874 e.V., Version 2.0 Institut Bauen und Umwelt e.V.,
DIN EN ISO 10874: 2012+A1:2021-04: Resilient, Berlin. www.ibu-epd.de
textile and laminate floor coverings - Classification
PCR Part A
ISO 14025 Product Category Rules for Construction Products
DIN EN /ISO 14025:2011-10/, Environmental labels from the range of Environmental Product Declarations.
and declarations — Type III environmental Part A: Calculation Rules for the Life Cycle
declarations — Principles and procedures Assessment and Requirements on the Background
Report, V1.9, Berlin: Institut Bauen und Umwelt e.V.
ISO 14040 (IBU), January 2021
DIN EN ISO 14040:2006+A1:2020 Environmental
management - Life cycle assessment - Principles and PCR Part B
framework Product Category Rules for Construction Products
from the range of Environmental Product Declarations
ISO 14044 of Institut Bauen und Umwelt (IBU),
DIN EN ISO 14044:2006+A1:2018+A2:2020 Part B: Requirements on the EPD for floor coverings,
Environmental management - Life cycle assessment - V1.2, Berlin: Institut Bauen und Umwelt e.V. (IBU),
Requirements and guidelines February 2018
ISO 15686 PRODIS
ISO 15686: Buildings and constructed assets - Product Information System (PRODIS) of the
Service life planning European Carpet Industry, Gemeinschaft
ISO 15686-1: 2011-05: Part 1: General principles and umweltfreundlicher Teppichboden e.V (GUT) and
framework European Carpet and Rug Association
ISO 15686-2: 2012-05: Part 2: Service life prediction (ECRA), http://www.pro-dis.info
procedures
ISO 15686-7: 2017-04: Part 7: Performance REACH
evaluation for feedback of service life data Regulation (EC) No 1907/2006 of the European
from practice Parliament and of the Council of 18 December 2006
ISO 15686-8: 2008-06: Part 8: Reference service life concerning the Registration, Evaluation, Authorisation
and service-life estimation and Restriction of Chemicals (REACH). Last update:
27.02.2020 (Status: 27.06.2018)
Regulation (EU) No. 305/2011
Regulation No. 305/2011 Construction Products VDZ e.V.
Regulation (CPR) of the European Council and of the Association of German Cement Works, Ed.
European Parliament, April 2011 Environmental Data of the German Cement Industry
2019
7 Environmental Product Declaration Balsan – NEXUS / NEXUS LINK - tufted carpet tiles
Publisher
Institut Bauen und Umwelt e.V. Tel +49 (0)30 3087748- 0
Panoramastr. 1 Fax +49 (0)30 3087748- 29
10178 Berlin Mail info@ibu-epd.com
Germany Web www.ibu-epd.com
Programme holder
Institut Bauen und Umwelt e.V. Tel +49 (0)30 - 3087748- 0
Panoramastr 1 Fax +49 (0)30 – 3087748 - 29
10178 Berlin Mail info@ibu-epd.com
Germany Web www.ibu-epd.com
Author of the Life Cycle
Assessment Tel +49 (0)241 96843 410
Gemeinschaft umweltfreundlicher Fax +49 (0)241 96843 400
Teppichboden (GUT) e.V. Mail mail@gut-ev.de
Schönebergstraße 2 Web www.gut-ev.org
52068 Aachen
Germany
Owner of the Declaration
Balsan Moquette Tel +33 (0) 254 2916 00
Corbilly 2 Fax +33 (0) 254 3679 08
36330 Arthon Mail cedric.charton@balsan.com
France Web www.balsan.com
