ENVIRONMENTAL PRODUCT DECLARATION
as per ISO 14025 and EN 15804+A2
Owner of the Declaration Kingspan Insulation B.V.
Publisher Institut Bauen und Umwelt e.V. (IBU)
Programme holder Institut Bauen und Umwelt e.V. (IBU)
Declaration number EPD-KIN-20230013-CBD1-EN
Issue date 07.02.2023
Valid to 06.02.2028
Therma™ TR27 / Therma™ TT47
Kingspan Insulation B.V.
www.ibu-epd.com | https://epd-online.com
General Information
Kingspan Insulation B.V. Therma™ TR27 / Therma™ TT47
Programme holder Owner of the declaration
IBU – Institut Bauen und Umwelt e.V. Kingspan Insulation B.V.
Hegelplatz 1 Lingewei 8
10117 Berlin 4004LL Tiel
Germany Netherlands
Declaration number Declared product / declared unit
EPD-KIN-20230013-CBD1-EN Therma™ TR27 / Therma™ TT47
1m2, 120mm thickness, R = 4,80 m2.K/W
D
This declaration is based on the product category rules: Scope:
Insulating materials made of foam plastics, 01.08.2021 The insulation materials Therma™ TR27 and Therma™ TT47 are
(PCR checked and approved by the SVR) produced by Kingspan Insulation at the manufacturing facilities in
Winterswijk (the Netherlands) and Burkhardtsdorf (Germany). This EPD is
based on weighted averages which have been determined on the basis of
Issue date the single values originating from the different Kingspan Insulation
factories.
07.02.2023
Therma™ TR27 Roof Board is an insulationboard with a rigid thermoset
polyisocyanurate (PIR) fibre-free insulation core, faced on both sides with
a mineral-coated glass tissue based facing. Therma™ TR27 Roof Board is
Valid to
used as thermal insulation under adherent, mechanically fixed or non-fixed
06.02.2028 ballasted roofing systems.
Therma™ TT47 Tapered Roof Board is an insulation board with a rigid
thermoset PIR fibre-free insulation core, faced on both sides with a
mineral-coated glass tissue based facing. Therma™ TT47 Tapered Roof
Board is used as thermal insulation under adherent, mechanically fixed or
non-fixed ballasted roofing systems and enhances water drainage from flat
roofs.
In order to enable the user of the EPD to calculate the LCA results for
different thicknesses, the EPD contains the respective calculation rules.
The owner of the declaration shall be liable for the underlying information
and evidence; the IBU shall not be liable with respect to manufacturer
information, life cycle assessment data and evidences.
Dipl.-Ing. Hans Peters
(Chairman of Institut Bauen und Umwelt e.V.)
The EPD was created according to the specifications of EN 15804+A2. In
the following, the standard will be simplified as EN 15804.
Verification
The standard EN 15804 serves as the core PCR
Independent verification of the declaration and data according to ISO
14025:2011
internally X externally
Florian Pronold Vito D'Incognito,
(Managing Director Institut Bauen und Umwelt e.V.) (Independent verifier)
1 Environmental Product Declaration - Kingspan Insulation B.V. - Therma™ TR27 / Therma™ TT47
Product
Performance data of the product in accordance with the
Product description/Product definition declaration of performance with respect to its essential
Therma™ TR27 and Therma™ TT47 Roof Boards are characteristics according to EN 13165 - Thermal insulation
insulation boards with a rigid thermoset polyisocyanurate (PIR) products for buildings - Factory made rigid polyurethane foam
fibre-free insulation core, faced on both sides with a mineral- (PU) products - Specification
coated glass tissue based facing. The products are available in The declaration of performance of the product can be found at
variable thicknesses from 20 mm up to 200 mm. This EPD is www.kingspan.com.
based on a thickness of 120 mm and R -value of 4,80 m²·K/W.
D
Base materials/Ancillary materials
For the placing on the market of the product in the European
Union/European Free Trade Association (EU/EFTA) (with the The product contains approximately 3,0 kg/m2 polyurethane
exception of Switzerland) Regulation (EU) No. 305/2011 (CPR) rigid foam and 0,6 kg/m2 coated glass tissue facings. The main
applies. The product needs a declaration of performance taking materials of the polyurethane foam are MDI (between 57-62 %),
into consideration EN 13165 - Thermal insulation products for polyol (between 27-32 %) and a blowing agent (between 5-6
buildings - Factory made polyurethane foam (PU) products - %). Due to the closed-cell structure (conform EN 13165), the
Specification and the CE-marking. For the application and use blowing agent remains in the foam. Water, flame retardants and
the respective national provisions apply. additives are added (between 4-8 %).
Application In the current REACH regulations, polyurethane foam insulation
Therma™ TR27 Roof Board is used as thermal insulation under products are considered 'articles' and are exempt from the
adherent, mechanically fixed or non-fixed ballasted roofing requirements of Articles 57 and 59(1) of REACH Regulation
systems. (EC) No 1907/2006. These products are not classified as
'hazardous products' according to any current legislation, and
Therma™ TT47 Tapered Roof Board is used as thermal can hence be declared as follows:
insulation under adherent, mechanically fixed or non-fixed - This article contains substances listed in the candidate list
ballasted roofing systems and enhances water drainage from (date: 31.08.2022) exceeding 0.1 percentage by mass: no.
flat roofs. - This article contains other carcinogenic, mutagenic, reprotoxic
(CMR) substances in categories 1A or 1B which are not on the
Technical Data
candidate list, exceeding 0.1 percentage by mass: no.
Constructional data - Biocide products were added to this construction product or it
has been treated with biocide products (this then concerns a
Name Value Unit
treated product as defined by the (EU) Biocidal Products
Thermal conductivity according to EN
0.027 W/(m.K) Regulation No. 528/2012
13165 for dN < 80mm
(BPR): no.
Thermal conductivity according to EN
0.026 W/(m.K)
13165 for dN 80 - 119mm Reference service life
Thermal conductivity according to EN The reference service life is not to be declared in this EPD as it
0.025 W/(m.K)
13165 for dN ≥ 120mm does not cover the use stage.
Reaction to fire according to EN 13165 E
Compressive strength according to EN CS(10\Y)
13165 120/150
Tensile strength according to EN 13165 TR80
Thickness tolerance according to EN
T2-T3
13165
LCA: Calculation rules
Declared Unit The environmental impacts have been calculated per plant over
The declared unit (1 m²) and conversion factors are listed in the the calendar year 2021. Based on the one-year production
table below. volume of Therma™ TR27 and Therma™ TT47 per plant, the
Declared unit individual environmental impacts are weighted.
Name Value Unit
The products Therma™ TR27 and Therma™ TT47 are grouped
Declared unit 1 m2 because they have the same composition. The shape of both
Gross density 30 kg/m3 products differs, as the Therma™ TR27 is a flat product and the
Grammage 3.6 kg/m2 Therma™ TT47 is a tapered product. The EPD is studied for a
common product thickness of 120 mm. Multiplication factors are
Layer thickness 0.12 m
included to calculate impacts for other product thicknesses
This EPD is based on a weighted average of the annual within the range of 20 to 200 mm.
production volume of two factories producing the products
Therma™ TR27 and/or Therma™ TT47.
System boundary
The scope of this EPD is the thermal insulation products The type of EPD according to EN 15804 is:
Therma™ TR27 and Therma™ TT47 as produced by Kingspan cradle to gate with options, modules C1–C4, and module D
Insulation at the manufacturing facilities in Winterswijk (the (A1–A3, C, D and additional modules:
Netherlands) and Burkhardtsdorf (Germany). A4, A5).
2 Environmental Product Declaration - Kingspan Insulation B.V. - Therma™ TR27 / Therma™ TT47
The product stage is a mandatory information module and it Geographic Representativeness
covers: Land or region, in which the declared product system is
· A1, raw material extraction and processing, processing of manufactured, used or handled at the end of the product´s
secondary material input (e.g. recycling processes), lifespan: Europe
· A2, transport to the manufacturer,
· A3, manufacturing, including provision of all materials,
Comparability
products and energy, packaging processing and its transport,
Basically, a comparison or an evaluation of EPD data is only
as well as waste processing up to the end-of-waste state or
possible if all the data sets to be compared were created
disposal of final residues during the product stage.
according to EN 15804 and the building context, respectively
the product-specific characteristics of performance, are taken
The construction process stage includes:
into account.
· A4 transport to the building site;
· A5 installation in the building including provision of all
Background database
materials, products and energy, as well as waste processing up
Background data from GaBi ts Version 10 is used with GaBi
to the end-of-waste state or disposal of final residues during the
data sets CUP2022.1.
construction process stage.
Factors for different thicknesses
The end-of-life stage is a mandatory information module and it
The LCA results for the insulation material declared in this EPD
covers:
refer to a product with a thickness of 120 mm.
· C1 de-construction, demolition;
To enable the user of the EPD to calculate the results for
· C2 transport to waste processing;
different thicknesses the factors in the following table can be
· C3 waste processing for reuse, recovery and/or recycling;
used for the calculation. The LCA results in chapter 5 have to
· C4 disposal (not applicable for this EPD) including provision
be multiplied by these factors.
and all transport, provision of all materials, products and related
energy and water use.
The scaling factors are applicable for the complete product,
where the facings are for all product thicknesses equal and the
Environmental burden of the incineration (R1 > 60 %) of the
foam inputs are scaling upwards and downwards with other
product at the end-of-life stage are assigned to the product
product thicknesses.
system (C3); resulting potential credits for thermal and electrical
energy from energy substitution are declared in module D.
LCA: Scenarios and additional technical information
Name Value Unit
Characteristic product properties of biogenic carbon
Litres of fuel 0.0103 l/100km
The total mass of biogenic carbon containing materials is less
Transport distance 100 km
than 5 % of the total mass of the product and accompanying
packaging. Gross density of products transported 30 kg/m3
Technical information
The following technical information is a basis for the declared Installation into the building (A5)
modules or can be used for developing specific scenarios in the Name ValueUnit
context of a building assessment. Total output substances following waste treatment
0.102 kg
on-site packaging material
Manufacturing (A3)
The recycling of the packaging is considered in A5.
A polyethylene packaging foil is used. The products are
transported on expanded polystyrene (EPS) skids.
Within Module A3 the following packaging of the final product is End of life (C1-C4)
included: The assumptions for C1 are: diesel driven excavator (100 kW;
- Polyethylene cover and wrap: 0,051 kg/m² - Expanded 0.2 litre fuel per ton excavated material). The assumptions for
Polystyrene skid: 0,051 kg/m² C2 are: Truck Euro 6, diesel driven, 26-28 t gross weight,
Transport to the building site (A4) assumed distance 50 km
3 Environmental Product Declaration - Kingspan Insulation B.V. - Therma™ TR27 / Therma™ TT47
Name Value Unit scenario information
Waste incineration with energy recuperation is assumed as an
Collected as mixed construction waste 3.6 kg
end-of-life scenario.
Energy recovery 3.6 kg
Reuse, recovery and/or recycling potentials (D), relevant
4 Environmental Product Declaration - Kingspan Insulation B.V. - Therma™ TR27 / Therma™ TT47
LCA: Results
DESCRIPTION OF THE SYSTEM BOUNDARY (X = INCLUDED IN LCA; ND = MODULE OR INDICATOR NOT DECLARED; MNR =
MODULE NOT RELEVANT)
Benefits and
Construction loads beyond
Product stage Use stage End of life stage
process stage the system
boundaries
la ire ta m w a Ry lp p u s tro p s n a rT g n iru tc a fu n a M e h t m o rf tro p s n a rTe tis e h t o t e ta g y lb m e s s A e s U e c n a n e tn ia M ria p e R tn e m e c a lp e R tn e m h s ib ru fe R y g re n e la n o ita re p Oe s u re ta w la n o ita re p Oe s u n o itc u rts n o c -e Dn o itilo m e d tro p s n a rT g n is s e c o rp e ts a W la s o p s iD -e s u e R-y re v o c e R-g n ilc y c e Rla itn e to p
A1 A2 A3 A4 A5 B1 B2 B3 B4 B5 B6 B7 C1 C2 C3 C4 D
X X X X X MND MND MNR MNR MNR MND MND X X X X X
RESULTS OF THE LCA - ENVIRONMENTAL IMPACT according to EN 15804+A2: 1m2 120mm Therma™ TR27 / Therma™ TT47
Parameter Unit A1-A3 A4 A5 C1 C2 C3 C4 D
GWP-total kg CO 2 eq 9.52E+00 3.03E-02 2.55E-01 2.31E-03 1.52E-02 7.19E+00 0 -2.86E+00
GWP-fossil kg CO 2 eq 9.56E+00 3.02E-02 2.55E-01 2.31E-03 1.51E-02 7.19E+00 0 -2.85E+00
GWP-biogenic kg CO 2 eq -4.14E-02 -4.17E-05 1.39E-05 3.09E-06 -2.09E-05 5.06E-04 0 -1.46E-02
GWP-luluc kg CO 2 eq 6.18E-03 1.68E-04 3.03E-06 2.85E-08 8.42E-05 3.35E-05 0 -3.13E-04
ODP kg CFC11 eq 2.37E-11 1.81E-15 4.54E-14 1.42E-16 9.05E-16 6.16E-13 0 -1.93E-11
AP mol H+ eq 2.06E-02 3.11E-05 3.18E-05 1.07E-05 1.56E-05 4.04E-03 0 -3.75E-03
EP-freshwater kg P eq 4.03E-05 9.01E-08 1.15E-08 4.65E-10 4.51E-08 2.61E-07 0 -3.92E-06
EP-marine kg N eq 5.18E-03 1.02E-05 8.53E-06 5.11E-06 5.09E-06 1.94E-03 0 -1.02E-03
EP-terrestrial mol N eq 5.39E-02 1.21E-04 1.45E-04 5.59E-05 6.06E-05 2.24E-02 0 -1.09E-02
kg NMVOC
POCP 2.55E-02 2.74E-05 2.46E-05 1.45E-05 1.37E-05 4.98E-03 0 -2.85E-03
eq
ADPE kg Sb eq 1.02E-05 2.52E-09 1.11E-09 9.44E-11 1.26E-09 1.69E-08 0 -4.3E-07
ADPF MJ 2.41E+02 4.04E-01 9.42E-02 3.12E-02 2.02E-01 2.05E+00 0 -4.85E+01
m3 world eq
WDP 1.44E+00 2.71E-04 2.42E-02 4.29E-06 1.35E-04 7.5E-01 0 -3.04E-01
deprived
GWP = Global warming potential; ODP = Depletion potential of the stratospheric ozone layer; AP = Acidification potential of land and water; EP =
Eutrophication potential; POCP = Formation potential of tropospheric ozone photochemical oxidants; ADPE = Abiotic depletion potential for non-fossil
resources; ADPF = Abiotic depletion potential for fossil resources; WDP = Water (user) deprivation potential)
RESULTS OF THE LCA - INDICATORS TO DESCRIBE RESOURCE USE according to EN 15804+A2: 1m2 120mm Therma™
TR27 / Therma™ TT47
Parameter Unit A1-A3 A4 A5 C1 C2 C3 C4 D
PERE MJ 2.1E+01 2.29E-02 2.42E-02 1.18E-04 1.15E-02 3.78E-01 0 -1.33E+01
PERM MJ 0 0 0 0 0 0 0 0
PERT MJ 2.1E+01 2.29E-02 2.42E-02 1.18E-04 1.15E-02 3.78E-01 0 -1.33E+01
PENRE MJ 1.21E+02 4.05E-01 4.33E+00 3.13E-02 2.02E-01 1.18E+02 0 -4.85E+01
PENRM MJ 1.2E+02 0 -4.24E+00 0 0 -1.16E+02 0 0
PENRT MJ 2.41E+02 4.05E-01 9.42E-02 3.13E-02 2.02E-01 2.05E+00 0 -4.85E+01
SM kg 0 0 0 0 0 0 0 0
RSF MJ 0 0 0 0 0 0 0 0
NRSF MJ 0 0 0 0 0 0 0 0
FW m3 6.35E-02 2.59E-05 5.75E-04 1.78E-07 1.3E-05 1.76E-02 0 -1.28E-02
PERE = Use of renewable primary energy excluding renewable primary energy resources used as raw materials; PERM = Use of renewable primary
energy resources used as raw materials; PERT = Total use of renewable primary energy resources; PENRE = Use of non-renewable primary energy
excluding non-renewable primary energy resources used as raw materials; PENRM = Use of non-renewable primary energy resources used as raw
materials; PENRT = Total use of non-renewable primary energy resources; SM = Use of secondary material; RSF = Use of renewable secondary fuels;
NRSF = Use of non-renewable secondary fuels; FW = Use of net fresh water
RESULTS OF THE LCA – WASTE CATEGORIES AND OUTPUT FLOWS according to EN 15804+A2:
1m2 120mm Therma™ TR27 / Therma™ TT47
Parameter Unit A1-A3 A4 A5 C1 C2 C3 C4 D
HWD kg 7.82E-08 1.94E-12 7.85E-12 1.03E-13 9.69E-13 2.62E-10 0 -6.56E-09
NHWD kg 2.38E-01 5.8E-05 2.29E-02 2.93E-06 2.9E-05 2.4E-01 0 -2.45E-02
RWD kg 2.64E-03 4.98E-07 3.92E-06 3.43E-08 2.49E-07 8.66E-05 0 -3.82E-03
CRU kg 0 0 0 0 0 0 0 0
MFR kg 0 0 0 0 0 0 0 0
MER kg 0 0 1.02E-01 0 0 3.6E+00 0 0
EEE MJ 0 0 4.63E-01 0 0 1.24E+01 0 0
EET MJ 0 0 8.29E-01 0 0 2.22E+01 0 0
5 Environmental Product Declaration - Kingspan Insulation B.V. - Therma™ TR27 / Therma™ TT47
HWD = Hazardous waste disposed; NHWD = Non-hazardous waste disposed; RWD = Radioactive waste disposed; CRU = Components for re-use;
MFR = Materials for recycling; MER = Materials for energy recovery; EEE = Exported electrical energy; EET = Exported thermal energy
RESULTS OF THE LCA – additional impact categories according to EN 15804+A2-optional:
1m2 120mm Therma™ TR27 / Therma™ TT47
Parameter Unit A1-A3 A4 A5 C1 C2 C3 C4 D
Disease
PM 1.67E-07 1.8E-10 3.88E-10 1.21E-10 8.98E-11 1.4E-08 0 -3.11E-08
incidence
IR kBq U235 eq 2.95E-01 7.3E-05 5.38E-04 4.99E-06 3.65E-05 1.38E-02 0 -6.47E-01
ETP-fw CTUe 9.77E+01 2.8E-01 6.74E-02 2.17E-02 1.4E-01 8.36E-01 0 -1.07E+01
HTP-c CTUh 6.64E-09 5.65E-12 3.78E-12 4.02E-13 2.82E-12 5.43E-11 0 -4.89E-10
HTP-nc CTUh 5.18E-07 2.93E-10 3.83E-10 2.03E-11 1.47E-10 2.25E-09 0 -1.88E-08
SQP SQP 3.68E+01 1.39E-01 2.41E-02 8.61E-05 6.94E-02 4.6E-01 0 -8.65E+00
PM = Potential incidence of disease due to PM emissions; IR = Potential Human exposure efficiency relative to U235; ETP-fw = Potential comparative
Toxic Unit for ecosystems; HTP-c = Potential comparative Toxic Unit for humans (cancerogenic); HTP-nc = Potential comparative Toxic Unit for humans
(not cancerogenic); SQP = Potential soil quality index
Disclaimer 1 – for the indicator “Potential Human exposure efficiency relative to U235”. This impact category deals mainly with the
eventual impact of low-dose ionizing radiation on human health of the nuclear fuel cycle. It does not consider effects due to possible
nuclear accidents, occupational exposure or radioactive waste disposal in underground facilities. Potential ionizing radiation from the
soil, radon and from some construction materials is also not measured by this indicator.
Disclaimer 2 – for the indicators “abiotic depletion potential for non-fossil resources”, “abiotic depletion potential for fossil resources”,
“water (user) deprivation potential, deprivation-weighted water consumption”, “potential comparative toxic unit for ecosystems”,
“potential comparative toxic unit for humans – cancerogenic”, “Potential comparative toxic unit for humans - not cancerogenic”,
“potential soil quality index”. The results of this environmental impact indicator shall be used with care as the uncertainties on these
results are high as there is limited experience with the indicator.
This EPD was created using a software tool.
References
Biocidal Products Regulation No. 528/2012 (BPR) EPD programme of Institut Bauen und Umwelt e.V., Version
Regulation (EU) No 528/2012 of the European Parliament and 2.0, Berlin: Institut Bauen und Umwelt e.V., 2021. www.ibu-
of the Council of 22 May 2012 concerning the making available epd.com
on the market and use of biocidal products
LCA-tool
CPR Kingspan LCA tool, version 1.1. IBU-KSI-202001-LT1- EN.
Regulation (EU) No. 305/2011 of the European Parliament and Developed by Sphera Solutions GmbH (formely Thinkstep
of the Council of 9 March 2011 laying down harmonised GmbH)
condition for the marketing of construction products and
repealing Council Directive 89/106/EC PCR Version 1.7, Part A
Institut Bauen und Umwelt e.V., Berlin (pub.): Product Category
ISO 14025 Rules for Building-Related Products and services, Part A:
EN ISO 14025:2011, Environmental labels and declarations — Calculation Rules for the Life Cycle Assessment and
Type III environmental declarations — Principles and Requirements on the Project Report according to EN
procedures. 15804+A2:2019 November 2021
EN 13165 PCR 2017, Part B
EN 13165:2012+A2:2016: Thermal insulation products for Institut Bauen und Umwelt e.V., Berlin (pub.): Product Category
buildings. Factory made polyurethane foam (PU) products. Rules for Construction Products from the range of
Specification Environmental Product Declarations of Institut Bauen und
Umwelt (IBU), Part B: Requirements on the EPD for insulating
EN 15804 materials made of foam plastics. January 2019
EN 15804:2012+A2:2019+AC:2021, Sustainability of
construction works — Environmental Product Declarations — REACH
Core rules for the product category of construction products. Regulation (EC) No 1907/2006 of the European Parliament and
of the Council on the Registration, Evaluation, Authorisation
GaBi ts and Restriction of Chemicals (REACH)
thinkstep AG: Leinfelden-Echterdingen GaBi Software- System https://echa.europa.eu/candidate-list-table;
and Database for Life Cycle Engineering 1992- 2019
Candidate list
IBU 2021 https://echa.europa.eu/candidate-list-table; accessed
Institut Bauen und Umwelt e.V.: General Instructions for the 31.08.2022, 233 substances listed.
6 Environmental Product Declaration - Kingspan Insulation B.V. - Therma™ TR27 / Therma™ TT47
Publisher
Institut Bauen und Umwelt e.V. +49 (0)30 3087748- 0
Hegelplatz 1 info@ibu-epd.com
10117 Berlin www.ibu-epd.com
Germany
Programme holder
Institut Bauen und Umwelt e.V. +49 (0)30 3087748- 0
Hegelplatz 1 info@ibu-epd.com
10117 Berlin www.ibu-epd.com
Germany
Author of the Life Cycle Assessment
Kingspan Insulation B.V. +31 (0) 543 543 210
Lingewei 8 info@kingspaninsulation.nl
4004LL Tiel www.kingspan.com
Netherlands
Owner of the Declaration
Kingspan Insulation B.V. +31 (0) 543 543 210
Lingewei 8 info@kingspaninsulation.nl
4004LL Tiel www.kingspan.com
Netherlands
7 Environmental Product Declaration - Kingspan Insulation B.V. - Therma™ TR27 / Therma™ TT47
