ENVIRONMENTAL PRODUCT DECLARATION
as per ISO 14025 and EN 15804+A2
Owner of the Declaration dormakaba International Holding GmbH
Publisher Institut Bauen und Umwelt e.V. (IBU)
Programme holder Institut Bauen und Umwelt e.V. (IBU)
Declaration number EPD-DOR-20230097-CBA1-EN
Issue date 22.06.2023
Valid to 21.06.2028
Digital cylinder
dormakaba
www.ibu-epd.com | https://epd-online.com
General Information
dormakaba Digital cylinder
Programme holder Owner of the declaration
IBU – Institut Bauen und Umwelt e.V. dormakaba International Holding GmbH
Hegelplatz 1 DORMA Platz 1
10117 Berlin 58256 Ennepetal
Germany Germany
Declaration number Declared product / declared unit
EPD-DOR-20230097-CBA1-EN 1 piece of the product: Digital cylinder, consisting of the following items:
• Digital cylinder
• Battery
• Assembly screw
• Product packaging
This declaration is based on the product category rules: Scope:
Building Hardware products, 01.08.2021 This EPD refers to a specific product manufactured by dormakaba. The
(PCR checked and approved by the SVR) production site is located in Wetzikon (Switzerland). Renewable electricity
is being used at this production site.
Issue date The owner of the declaration shall be liable for the underlying information
and evidence; the IBU shall not be liable with respect to manufacturer
22.06.2023
information, life cycle assessment data and evidences.
The EPD was created according to the specifications of EN 15804+A2. In
Valid to
the following, the standard will be simplified as EN 15804.
21.06.2028
Verification
The standard EN 15804 serves as the core PCR
Independent verification of the declaration and data according to ISO
14025:2011
internally X externally
Dipl.-Ing. Hans Peters
(Chairman of Institut Bauen und Umwelt e.V.)
Florian Pronold Matthias Klingler,
(Managing Director Institut Bauen und Umwelt e.V.) (Independent verifier)
1 Environmental Product Declaration - dormakaba - Digital cylinder
Product
The products are not harmonized in accordance with the
Product description/Product definition Construction Product Regulations (CPR) but in accordance with
The products are mechatronic cylinder locks with both visual other provisions for harmonization of the EU. Compliance with
and acoustic access signals. They are compact, energy- the European Union Directive and technical specifications:
efficient and easy to install. The many different versions offer a
• Directive 2014/53/EU (RED)
solution for every door. The digital cylinder is part of the
• Directive (EU) No 2011/65 (RoHS)
dormakaba evolo standalone portfolio. That means no cabling
• Regulation (EC) No 1907/2006 (REACH)
is required within the door because it is operated with a
• EN 15684 (Mechatronic Cylinders)
standard battery. The modular design of the digital cylinder with
The products are subject to CE marking according to the
removable knobs enables quick and easy installation. For the
relevant harmonization legislation.
placing on the market in the European Union/European Free
Trade Association (EU/EFTA) (with the exception of Base materials/Ancillary materials
Switzerland) the following legal provisions apply:
The composition of the product including the packaging is listed
• Radio Equipment Directive (RED) below:
• Restriction of Hazardous Substances (RoHS) Name Value Unit
The CE-marking considers the proof of conformity with the
Brass 45 %
respective harmonized standards based on the legal provisions
Zinc 23 %
above. For the application and use the respective national
provisions apply. Copper 9 %
Paper 9 %
Application
Plastics 4 %
The product can be installed in any internal or external door
Battery and electronics 4 %
made of wood, glass or metal. It is also suitable for installation
in fire doors. Stainless steel 3 %
Steel 3 %
Technical Data
The product/s include/s partial articles which contain
The digital cylinder has the following technical properties:
substances listed in the Candidate List of REACH Regulation
Name Value Unit
1907/2006/EC (date: 17.01.2023) exceeding 0.1 percentage by
Dimensions cylinder length from 25/20 mm mass: yes
to max. cylinder length 220 mm
External knob 36 x 45 mm • Lead (Pb): 7439-92-1 (CAS-No.)
is included in some of the alloys used. The
Internal knob 36 x 29 mm
concentration of lead in each individual alloy does not
Small internal knob 30 x 27 mm
exceed 4.0 % (by mass).
Temperature -25 to +70 °C The Candidate List can be found on the ECHA website
Protection class of external address: https://echa.europa.eu/de/home.
IP56
knob
Reference service life
Corrosion resistance Class 3 EN 1670
The reference service life of the Digital cylinders amounts to 10
up to 50.000 or up to 2
Battery service life at 20 °C years and depends on the application and frequency of use.
cylces years
For repairs or renewals, suitable spare parts are available. The
Weight (60 mm length) 0,4 kg
product is certified to EN 15684, meaning it is designed to
withstand a minimum of 100.000 uses.
LCA: Calculation rules
mechanical treatments, including provision of all materials,
Declared Unit products and energy, as well as waste processing up to the
The declared unit is 1 piece of the product including the end-of waste state.
packaging: Digital cylinder.
Name Value Unit Construction stage - Modules A4-A5
Declared unit 1 piece/product The construction process stage includes:
— A4, transport to the building site;
Mass (including packaging) 0,45 kg
— A5, treatment of waste packaging materials arising during
installation into the building.
System boundary
The type of EPD is according to EN 15804: "cradle to gate with
Maintenance – Module B2
options, modules C1–C4,
This module includes the production and the end of life of the
and module D". The following modules are declared: A1-A3, C,
batteries. The potential use of batteries is declared in module
D and additional modules: A4 + A5 + B6
B2.
Production - Module A1-A3
The product stage includes:
— A1, raw material extraction, processing of secondary
material input (e.g. recycling processes);
— A2, transport to the manufacturer;
— A3, manufacturing and assembly, processing and
2 Environmental Product Declaration - dormakaba - Digital cylinder
End-of-life stage– Modules C1-C4 and D
The end-of-life stage includes: Geographic Representativeness
— C1, de-construction, demolition; Land or region, in which the declared product system is
— C2, transport to waste processing; manufactured, used or handled at the end of the product´s
— C3, waste processing for reuse, recovery and/or recycling; lifespan: Europe
— C4, disposal;
including provision and all transport, provision of all materials,
Comparability
products and related energy and water use.
Basically, a comparison or an evaluation of EPD data is only
— D, recycling potentials, expressed as net impacts and
possible if all the data sets to be compared were created
benefits.
according to EN 15804 and the building context, respectively
the product-specific characteristics of performance, are taken
into account. Background database: GaBi, SP40.
LCA: Scenarios and additional technical information
dormakaba digital cylinders are operated using a battery and
Characteristic product properties of biogenic carbon are not connected to mains electricity. The battery is provided
Information on describing the biogenic Carbon Content at by dormakaba. During the operation of the product, the only
factory gate energy consumption comes from the battery use. The battery
must be exchanged in average ten times over the declared
Name ValueUnit
service life.
Biogenic carbon content in accompanying kg
0.01
packaging C
Note: 1 kg of biogenic carbon is equivalent to 44/12 kg of CO 2. Reference service life
Name Value Unit
Life Span according to the manufacturer 10 a
End of life (C1-C4)
Transport to the building site (A4) C1: The product dismantling from the building is done manually
Name Value Unit without environmental burden.
C2: Transport to waste treatment at end of life is 50 km.
Litres of fuel 0.00276 l/100km
Name Value Unit
Transport distance 100 km
Recycling 37 kg
Capacity utilisation (including empty runs) 55 %
Energy recovery 0.02 kg
The product is transported via truck. The main distribution
Landfilling 0.02 kg
region is Europe. In order to allow scaling to a specific point of
installation via truck, 100 km are declared. Transportation to Waste Processing Site 50 km
Reuse, recovery and/or recycling potentials (D), relevant
Installation into the building (A5)
scenario information
Name Value Unit
Name Value Unit
Waste (paper packaging) 0.04 kg
Recycling 100 %
Maintenance (B2) The collection rate is 100 %.
Name Value Unit
Number of batteries required for lifetime 10 pcs.
3 Environmental Product Declaration - dormakaba - Digital cylinder
LCA: Results
DESCRIPTION OF THE SYSTEM BOUNDARY (X = INCLUDED IN LCA; MND = MODULE OR INDICATOR NOT DECLARED; MNR
= MODULE NOT RELEVANT)
Benefits and
Construction loads beyond
Product stage Use stage End of life stage
process stage the system
boundaries
la ire ta m w a Ry lp p u s tro p s n a rT g n iru tc a fu n a M e h t m o rf tro p s n a rTe tis e h t o t e ta g y lb m e s s A e s U e c n a n e tn ia M ria p e R tn e m e c a lp e R tn e m h s ib ru fe R y g re n e la n o ita re p Oe s u re ta w la n o ita re p Oe s u n o itc u rts n o c -e Dn o itilo m e d tro p s n a rT g n is s e c o rp e ts a W la s o p s iD -e s u e R-y re v o c e R-g n ilc y c e Rla itn e to p
A1 A2 A3 A4 A5 B1 B2 B3 B4 B5 B6 B7 C1 C2 C3 C4 D
X X X X X MND X MNR MNR MNR MND MND X X X X X
RESULTS OF THE LCA - ENVIRONMENTAL IMPACT according to EN 15804+A2: 1 piece Digital cylinder
Parameter Unit A1-A3 A4 A5 B2 C1 C2 C3 C4 D
GWP-total kg CO 2 eq 2.85E+00 3.94E-03 5.67E-02 1.72E-01 0 1.8E-03 4.83E-02 2.7E-04 -8.21E-01
GWP-fossil kg CO 2 eq 2.91E+00 3.76E-03 1.42E-03 1.71E-01 0 1.72E-03 4.83E-02 2.68E-04 -8.2E-01
GWP-biogenic kg CO 2 eq -5.88E-02 1.74E-04 5.53E-02 3.17E-04 0 7.94E-05 1.13E-06 9.17E-07 -4.94E-04
GWP-luluc kg CO 2 eq 2.42E-03 8.95E-08 9.33E-07 1.65E-04 0 4.09E-08 2.73E-06 7.73E-07 -7.55E-04
ODP kg CFC11 eq 2.81E-11 3.97E-19 1.02E-17 3.23E-12 0 1.81E-19 2.44E-17 9.96E-19 -3.31E-15
AP mol H+ eq 1.91E-02 3.76E-06 1.59E-05 5.36E-04 0 1.72E-06 8.6E-06 1.93E-06 -8.61E-03
EP-freshwater kg P eq 6.86E-06 8.05E-10 2E-09 2.76E-07 0 3.68E-10 3.88E-09 4.61E-10 -1.2E-06
EP-marine kg N eq 2.44E-03 1.2E-06 5.73E-06 1.18E-04 0 5.47E-07 1.94E-06 4.96E-07 -9E-04
EP-terrestrial mol N eq 2.65E-02 1.33E-05 7.15E-05 1E-03 0 6.08E-06 3.92E-05 5.45E-06 -9.74E-03
kg NMVOC
POCP 7.49E-03 3.39E-06 1.52E-05 3.22E-04 0 1.55E-06 5.36E-06 1.5E-06 -2.95E-03
eq
ADPE kg Sb eq 8.11E-04 1.13E-10 1.61E-10 7.54E-07 0 5.15E-11 3.34E-10 2.41E-11 -4.43E-04
ADPF MJ 4.08E+01 5.33E-02 1.79E-02 2.21E+00 0 2.44E-02 2.24E-02 3.52E-03 -9.57E+00
m3 world eq
WDP 6.92E-01 7.37E-06 7.03E-03 2.3E-02 0 3.37E-06 4.94E-03 2.81E-05 -2.28E-01
deprived
GWP = Global warming potential; ODP = Depletion potential of the stratospheric ozone layer; AP = Acidification potential of land and water; EP =
Eutrophication potential; POCP = Formation potential of tropospheric ozone photochemical oxidants; ADPE = Abiotic depletion potential for non-fossil
resources; ADPF = Abiotic depletion potential for fossil resources; WDP = Water (user) deprivation potential)
RESULTS OF THE LCA - INDICATORS TO DESCRIBE RESOURCE USE according to EN 15804+A2: 1 piece Digital cylinder
Parameter Unit A1-A3 A4 A5 B2 C1 C2 C3 C4 D
PERE MJ 1.37E+01 1.68E-04 4.83E-01 4.45E-01 0 7.68E-05 5.82E-03 4.61E-04 -1.57E+00
PERM MJ 4.8E-01 0 -4.8E-01 0 0 0 0 0 0
PERT MJ 1.42E+01 1.68E-04 3.25E-03 4.45E-01 0 7.68E-05 5.82E-03 4.61E-04 -1.57E+00
PENRE MJ 4.03E+01 5.34E-02 1.79E-02 2.21E+00 0 2.44E-02 6.68E-01 3.52E-03 -9.57E+00
PENRM MJ 6.46E-01 0 0 0 0 0 -6.46E-01 0 0
PENRT MJ 4.1E+01 5.34E-02 1.79E-02 2.21E+00 0 2.44E-02 2.24E-02 3.52E-03 -9.57E+00
SM kg 2.35E-01 0 0 0 0 0 0 0 0
RSF MJ 0 0 0 0 0 0 0 0 0
NRSF MJ 0 0 0 0 0 0 0 0 0
FW m3 1.82E-02 3.02E-07 1.66E-04 9.99E-04 0 1.38E-07 1.18E-04 8.88E-07 -5.96E-03
PERE = Use of renewable primary energy excluding renewable primary energy resources used as raw materials; PERM = Use of renewable primary
energy resources used as raw materials; PERT = Total use of renewable primary energy resources; PENRE = Use of non-renewable primary energy
excluding non-renewable primary energy resources used as raw materials; PENRM = Use of non-renewable primary energy resources used as raw
materials; PENRT = Total use of non-renewable primary energy resources; SM = Use of secondary material; RSF = Use of renewable secondary fuels;
NRSF = Use of non-renewable secondary fuels; FW = Use of net fresh water
RESULTS OF THE LCA – WASTE CATEGORIES AND OUTPUT FLOWS according to EN 15804+A2:
1 piece Digital cylinder
Parameter Unit A1-A3 A4 A5 B2 C1 C2 C3 C4 D
HWD kg 2.77E-07 5.18E-12 2.64E-11 2.77E-08 0 2.37E-12 8.53E-11 5.37E-11 -1.44E-07
NHWD kg 2.37E-01 5.46E-06 1.78E-03 4.2E-02 0 2.49E-06 5.02E-03 1.77E-02 -5.71E-02
RWD kg 1.82E-03 5.73E-08 9.41E-07 5.14E-05 0 2.62E-08 8.31E-07 4.01E-08 -3.05E-04
CRU kg 0 0 0 0 0 0 0 0 0
MFR kg 0 0 0 0 0 0 3.74E-01 0 0
MER kg 0 0 0 0 0 0 0 0 0
EEE MJ 0 0 8.58E-02 0 0 0 9.2E-02 0 0
EET MJ 0 0 1.56E-01 0 0 0 2.11E-01 0 0
4 Environmental Product Declaration - dormakaba - Digital cylinder
HWD = Hazardous waste disposed; NHWD = Non-hazardous waste disposed; RWD = Radioactive waste disposed; CRU = Components for re-use;
MFR = Materials for recycling; MER = Materials for energy recovery; EEE = Exported electrical energy; EET = Exported thermal energy
RESULTS OF THE LCA – additional impact categories according to EN 15804+A2-optional:
1 piece Digital cylinder
Parameter Unit A1-A3 A4 A5 B2 C1 C2 C3 C4 D
Disease
PM 1.77E-07 1.98E-11 8.8E-11 5.63E-09 0 9.04E-12 1.1E-10 2.38E-11 -8.15E-08
incidence
IR kBq U235 eq 1.99E-01 8.19E-06 1.46E-04 5E-03 0 3.74E-06 7.49E-05 4.13E-06 -3.59E-02
ETP-fw CTUe 3.14E+01 3.78E-02 8.5E-03 7.55E+00 0 1.73E-02 8.4E-03 2.01E-03 -4.21E+00
HTP-c CTUh 1.93E-08 7.11E-13 4.49E-13 3.83E-11 0 3.25E-13 7.27E-13 2.98E-13 1.1E-09
HTP-nc CTUh 1.01E-07 3.04E-11 1.95E-11 4.44E-09 0 1.39E-11 7.36E-11 3.29E-11 1.46E-07
SQP SQP 1.82E+01 1.37E-04 4.75E-03 2.15E-01 0 6.26E-05 6.71E-03 7.34E-04 -2.09E+00
PM = Potential incidence of disease due to PM emissions; IR = Potential Human exposure efficiency relative to U235; ETP-fw = Potential comparative
Toxic Unit for ecosystems; HTP-c = Potential comparative Toxic Unit for humans (cancerogenic); HTP-nc = Potential comparative Toxic Unit for humans
(not cancerogenic); SQP = Potential soil quality index
Disclaimer 1 – for the indicator 'Potential Human exposure efficiency relative to U235'. This impact category deals mainly with the
eventual impact of low-dose ionizing radiation on human health of the nuclear fuel cycle. It does not consider effects due to possible
nuclear accidents, occupational exposure nor due to radioactive waste disposal in underground facilities. Potential ionizing radiation
from the soil, from radon and from some construction materials is also not measured by this indicator.
Disclaimer 2 – for the indicators 'abiotic depletion potential for non-fossil resources', 'abiotic depletion potential for fossil resources',
'water (user) deprivation potential, deprivation-weighted water consumption', 'potential comparative toxic unit for ecosystems', 'potential
comparative toxic unit for humans – cancerogenic', 'Potential comparative toxic unit for humans - not cancerogenic', 'potential soil
quality index'. The results of this environmental impact indicator shall be used with care as the uncertainties on these results are high
or as there is limited experienced with the indicator.
This EPD was created using a software tool.
References
ISO 14025
DIN EN ISO 14025:2011-10, Environmental labels and GaBi ts software
declarations — Type III environmental Sphera Solutions GmbH
declarations — Principles and procedures Gabi Software System and Database for Life Cycle Engineering
1992-2020 Version 10.0.0.71
EN 15684 University of Stuttgart
EN 15684:2021-05, Building hardware - Mechatronic cylinders - Leinfelden-Echterdingen
Requirements and test methods
GaBi ts documentation
EN 15804+A2 GaBi life cycle inventory data documentation (https://www.gabi-
EN 15804:2019+A2, Sustainability of construction software.com/support/gabi/gabi-database-2020-lci-
works — Environmental Product Declarations — Core documentation/)
rules for the product category of construction products
LCA-tool dormakaba
Radio Equipment Directive (RED) LCA tool, version 1.0, LCA-tool, IBU-DOR-202101-LT1-EN,
Directive 2014/53/EU of the European Parliament and of the developed by Sphera Solutions GmbH
Council of 16 April 2014 on the harmonisation of the laws of the
Member States relating to the making available on the market PCR Part A
of radio equipment and repealing Directive 1999/5/EC PCR – Part A: Calculation Rules for the Life Cycle As-sessment
and Requirements on the Project Re-port according to EN
Registration, Evaluation, Authorisation and Restriction of 15804+A2:2019, Version 1.0, Institut Bauen und Umwelt e.V.,
Chemicals (REACH) www.ibu-epd.com
Regulation (EC) No 1907/2006 of the European Parliament and
of the Council on the Registration, Evaluation, Authorisation PCR Part B
and Restriction of Chemicals (REACH) PCR – Part B: Requirements on the EPD for Building Hardware
product, version 1.2, Institut Bauen und Umwelt e.V., www.ibu-
Restriction of Hazardous Substances (RoHS) epd.com, 2017
Directive on the restriction of the use of certain hazardous
substances in electrical and electronic equipment (RoHS),
Directive (EU) No 2011/65
Further References
IBU 2021
Institut Bauen und Umwelt e.V.: General Instructions
for the EPDs programme of Institut Bauen und Umwelt
e.V. Version 2.0., Berlin: Institut Bauen und Umwelt
e.V., 2021. www.ibu-epd.com
5 Environmental Product Declaration - dormakaba - Digital cylinder
Publisher
Institut Bauen und Umwelt e.V. +49 (0)30 3087748- 0
Hegelplatz 1 info@ibu-epd.com
10117 Berlin www.ibu-epd.com
Germany
Programme holder
Institut Bauen und Umwelt e.V. +49 (0)30 3087748- 0
Hegelplatz 1 info@ibu-epd.com
10117 Berlin www.ibu-epd.com
Germany
Author of the Life Cycle Assessment
dormakaba International Holding GmbH +49 2333 793-0
DORMA Platz 1 info.de@dormakaba.com
58256 Ennepetal www.dormakaba.com
Germany
Owner of the Declaration
dormakaba International Holding GmbH +49 2333 793-0
DORMA Platz 1 info.de@dormakaba.com
58256 Ennepetal www.dormakaba.com
Germany
6 Environmental Product Declaration - dormakaba - Digital cylinder
