ENVIRONMENTAL PRODUCT DECLARATION
as per ISO 14025 and EN 15804+A2
Owner of the Declaration dormakaba International Holding GmbH
Publisher Institut Bauen und Umwelt e.V. (IBU)
Programme holder Institut Bauen und Umwelt e.V. (IBU)
Declaration number EPD-DOR-20230098-CBA1-EN
Issue date 13.04.2023
Valid to 12.04.2028
SafeRoute
dormakaba
www.ibu-epd.com | https://epd-online.com
General Information
dormakaba SafeRoute
Programme holder Owner of the declaration
IBU – Institut Bauen und Umwelt e.V. dormakaba International Holding GmbH
Hegelplatz 1 DORMA Platz 1
10117 Berlin 58256 Ennepetal
Germany Germany
Declaration number Declared product / declared unit
EPD-DOR-20230098-CBA1-EN 1 piece of the product: Escape Route Security System SafeRoute,
consisting of the following items:
• SafeRoute STL-G door terminal
• SafeRoute STV electromagnetic door looking device
• Product packaging
This declaration is based on the product category rules: Scope:
Building Hardware products, 01.08.2021 This Environment Product Declaration refers to a specific escape route
(PCR checked and approved by the SVR) security system manufactured by dormakaba. The production site is
located in Ennepetal (Germany). Green electricity is being used at this
production site.
Issue date
Data represents the year 2022.
13.04.2023
The owner of the declaration shall be liable for the underlying information
and evidence; the IBU shall not be liable with respect to manufacturer
information, life cycle assessment data and evidences.
Valid to
12.04.2028 The EPD was created according to the specifications of EN 15804+A2. In
the following, the standard will be simplified as EN 15804.
Verification
The standard EN 15804 serves as the core PCR
Independent verification of the declaration and data according to ISO
14025:2011
internally X externally
Dipl.-Ing. Hans Peters
(Chairman of Institut Bauen und Umwelt e.V.)
Florian Pronold Matthias Klingler,
(Managing Director Institut Bauen und Umwelt e.V.) (Independent verifier)
1 Environmental Product Declaration - dormakaba - SafeRoute
Product
SafeRoute includes partial articles which contain substances
Product description/Product definition listed in the Candidate List of REACH Regulation
SafeRoute is a modularly constructed escape route security 1907/2006/EC (date: 17.01.2023) exceeding 0.1 percentage by
system that convincingly interconnects the contrasting mass: yes
requirements of doors in emergency exits and escape routes to
• Lead (Pb): 7439-92-1 (CAS-No.) is used in some of the
save people's lives on the one hand, while securing property on
alloys. The concentration of lead in each individual alloy
the other hand.
does not exceed 4.0% (by mass).
The Candidate List can be found on the ECHA website
With escape routes, building regulations require doors to be
address: https://echa.europa.eu/de/home.
easily opened from inside without external tools. At the same
time, insurers, police and facility operators require the most Reference service life
secure lock possible against misuse and break-ins. For the use
The reference service life of the product amounts to 10 years
and application of the product the respective national provisions
and depends on the application and frequency of use. Regular
at the place of use apply. For SafeRoute the standards which
maintenance is advised to ensure the life expectancy of 10
can be applied are the following:
years. For repairs and renewals, suitable spare parts are
• EN 13637: 2015-12 available. The product is tested and certified to EN 13637,
• 2011/65/EU ROHS3 Directive meaning they are designed to withstand a minimum of 200.000
cycles.
Application
Doors in emergency exits are subject to many different
requirements. SafeRoute offers comprehensive functions and
options for securing emergency exits, which is why it features a
flexible and modular design. The spectrum of uses ranges from
simple retrofitting of a door to a secure escape route door.
Installation of a complex escape route system with central
monitoring and control via door management software or
central management centers is also possible.
Technical Data
The escape route security system has the following technical
properties:
Name Value Unit
Power supply
Version without a power via DCW bus 24 V DC +-
supply unit 10%
Version with a power supply above 230 V AC +- 10% 24
unit V DC
Output voltage 1A
Power input
Closed-circuit current 65 mA
During alarm 100 mA
Class of protection IP 32
Temperature range -10°C to +55 °C
up to 93% (non-
Rel. Humidity
condensing)
Dimensions (W x H x D) approx. 95 x 253 x 75 cm
Performance data of the product with respect to its
characteristics in accordance with the relevant technical
provision which can be applied are mentioned above.
Base materials/Ancillary materials
The major material composition including the packaging of the
product is listed below.
Name Value Unit
Steel 42 %
Paper 21 %
Zinc 17 %
Aluminium 6 %
Plastic 5 %
Electronics 5 %
Primer and paint 4 %
2 Environmental Product Declaration - dormakaba - SafeRoute
LCA: Calculation rules
Declared Unit Use stage - Module B6
The declared unit is 1 piece of the product: SafeRoute The use stage related to the operation of the building includes:
— B6, operational energy use
Name Value Unit
Declared unit 1 piece/product End-of-life stage– Modules C1-C4 and D
The end-of-life stage includes:
Mass of declared product including
5.32 kg — C1, de-construction, demolition:
packaging
— C2, transport to waste processing;
— C3, waste processing for reuse, recovery and/or recycling;
System boundary
— C4, disposal; including provision and all transport, provision
The type of EPD is: cradle to gate with options, modules C1–
of all materials, products and related energy and water use.
C4, and module D (A1–A3 + C + D and additional modules: A4
+ A5)
Module D (Benefits and loads beyond the system boundary)
includes:
Production - Module A1-A3
— D, recycling potentials, expressed as net impacts and
The product stage includes:
benefits.
— A1, raw material extraction, processing and mechanical
treatments, processing of secondary material input (e.g. Geographic Representativeness
recycling processes), — A2, transport to the manufacturer, Land or region, in which the declared product system is
— A3, manufacturing and assembly including provision of all manufactured, used or handled at the end of the product´s
materials, products and energy, as well as waste processing up lifespan: Germany
to the end-of waste state.
Construction stage - Modules A4-A5 Comparability
The construction process stage includes: Basically, a comparison or an evaluation of EPD data is only
— A4, transport to the building site; possible if all the data sets to be compared were created
— A5, installation into the building; according to EN 15804 and the building context, respectively
including provision of all materials, products and energy, as well the product-specific characteristics of performance, are taken
as waste processing up to the end-of waste state or disposal of into account.
final residues during the construction process stage.
LCA: Scenarios and additional technical information
Characteristic product properties of biogenic carbon
Reference service life
Information on describing the biogenic Carbon Content at
Name Value Unit
factory gate
Life Span according to the manufacturer 10 a
Name ValueUnit
kg Operational energy use (B6)
Biogenic carbon content in product 0.35
C Name ValueUnit
B paio cg ke an gi ic n gcarbon content in accompanying 0.055 k Cg E yele ac rtricity consumption STL G and STV 200 for 1 21.37 kWh
Note: 1 kg of biogenic carbon is equivalent to 44/12 kg of CO . Days per year in use 365 days
2
One mode per day 0,2 h
Idle mode per day 23,8 h
Additional technical information for the declared modules.
On mode power STL G 2,4 W
Transport to the building site (A4) On mode power STV 200 4,8 W
Name Value Unit Idle mode power STL G 1,2 W
Litres of fuel truck (per 1 kg) 0.00276 l/100km Idle mode power STV 200 1,2 W
Transport distance medium truck 100 km
End of life (C1-C4)
Capacity utilisation (including empty runs) 55 %
C1: The product dismantling from the building is done manually
The product is transported via truck. The product is stored in without environmental burden.
the dormakaba logistic center in Germany. The main
Name Value Unit
distribution region is Europe. In order to allow scaling to a
Collected separately waste type 5.17 kg
specific point of installation 100 km are declared.
Recycling 4.75 kg
Installation into the building (A5) Energy recovery 0.257 kg
Landfilling 0.16 kg
Name Value Unit
Transport to waste managment 50 km
Waste packaging (paper and plastic) 0,15 kg
3 Environmental Product Declaration - dormakaba - SafeRoute
The product is disassembled in a recycling process.
Material recycling is then assumed for the metals and
electronics. The plastic components are assumed to be
incinerated with energy recovery. Electromechanics and minor
proportions of residues arising from the recycling process are
landfilled.
Region for the End of Life is: Europe.
Reuse, recovery and/or recycling potentials (D), relevant
scenario information
Name Value Unit
Recycling 100 %
Collection rate is 100%.
4 Environmental Product Declaration - dormakaba - SafeRoute
LCA: Results
DESCRIPTION OF THE SYSTEM BOUNDARY (X = INCLUDED IN LCA; MND = MODULE OR INDICATOR NOT DECLARED; MNR
= MODULE NOT RELEVANT)
Benefits and
Construction loads beyond
Product stage Use stage End of life stage
process stage the system
boundaries
la ire ta m w a Ry lp p u s tro p s n a rT g n iru tc a fu n a M e h t m o rf tro p s n a rTe tis e h t o t e ta g y lb m e s s A e s U e c n a n e tn ia M ria p e R tn e m e c a lp e R tn e m h s ib ru fe R y g re n e la n o ita re p Oe s u re ta w la n o ita re p Oe s u n o itc u rts n o c -e Dn o itilo m e d tro p s n a rT g n is s e c o rp e ts a W la s o p s iD -e s u e R-y re v o c e R-g n ilc y c e Rla itn e to p
A1 A2 A3 A4 A5 B1 B2 B3 B4 B5 B6 B7 C1 C2 C3 C4 D
X X X X X MND MND MNR MNR MNR X MND X X X X X
RESULTS OF THE LCA - ENVIRONMENTAL IMPACT according to EN 15804+A2: 1 piece SafeRoute
Parameter Unit A1-A3 A4 A5 B6 C1 C2 C3 C4 D
GWP-total kg CO 2 eq 2.27E+01 4.7E-02 2.13E-01 8.64E+01 0 2.3E-02 2.89E+00 2E-03 -7.35E+00
GWP-fossil kg CO 2 eq 2.43E+01 4.4E-02 5E-03 8.6E+01 0 2.2E-02 1.19E+00 2E-03 -7.33E+00
GWP-biogenic kg CO 2 eq -1.68E+00 2E-03 2.07E-01 2.87E-01 0 1E-03 1.7E+00 8.29E-06 -1.5E-02
GWP-luluc kg CO 2 eq 3.2E-02 1.06E-06 3.5E-06 1.25E-01 0 5.24E-07 8.23E-05 6.99E-06 -4E-03
ODP kg CFC11 eq 1.87E-09 4.7E-18 3.83E-17 1.89E-12 0 2.33E-18 7.96E-16 9E-18 -1.65E-11
AP mol H+ eq 1.2E-01 4.45E-05 5.96E-05 1.9E-01 0 2.21E-05 4.54E-04 1.74E-05 -3.4E-02
EP-freshwater kg P eq 1.43E-04 9.52E-09 7.5E-09 2.3E-04 0 4.72E-09 1.25E-07 4.17E-09 -1.17E-05
EP-marine kg N eq 2.06E-02 1.42E-05 2.15E-05 4.2E-02 0 7.02E-06 1.27E-04 4.48E-06 -4E-03
EP-terrestrial mol N eq 2.14E-01 1.57E-04 2.68E-04 4.43E-01 0 7.8E-05 2E-03 4.92E-05 -4.6E-02
kg NMVOC
POCP 6.11E-02 4.01E-05 5.7E-05 1.16E-01 0 1.98E-05 3.48E-04 1.36E-05 -1.5E-02
eq
ADPE kg Sb eq 6.09E-03 1.33E-09 6.05E-10 2.49E-05 0 6.61E-10 1.14E-08 2.18E-10 -2E-03
ADPF MJ 3.18E+02 6.31E-01 6.7E-02 1.51E+03 0 3.12E-01 9.09E-01 3.2E-02 -9.84E+01
m3 world eq
WDP 6.05E+00 8.72E-05 2.6E-02 1.88E+01 0 4.32E-05 2.97E-01 2.54E-04 -1.18E+00
deprived
GWP = Global warming potential; ODP = Depletion potential of the stratospheric ozone layer; AP = Acidification potential of land and water; EP =
Eutrophication potential; POCP = Formation potential of tropospheric ozone photochemical oxidants; ADPE = Abiotic depletion potential for non-fossil
resources; ADPF = Abiotic depletion potential for fossil resources; WDP = Water (user) deprivation potential)
RESULTS OF THE LCA - INDICATORS TO DESCRIBE RESOURCE USE according to EN 15804+A2: 1 piece SafeRoute
Parameter Unit A1-A3 A4 A5 B6 C1 C2 C3 C4 D
PERE MJ 1.23E+02 2E-03 1.81E+00 6.7E+02 0 9.85E-04 1.16E+01 4E-03 -2.67E+01
PERM MJ 1.32E+01 0 -1.8E+00 0 0 0 -1.14E+01 0 0
PERT MJ 1.37E+02 2E-03 1.2E-02 6.7E+02 0 9.85E-04 2.09E-01 4E-03 -2.67E+01
PENRE MJ 3.07E+02 6.31E-01 6.7E-02 1.51E+03 0 3.13E-01 1.2E+01 3.2E-02 -9.84E+01
PENRM MJ 1.11E+01 0 0 0 0 0 -1.11E+01 0 0
PENRT MJ 3.18E+02 6.31E-01 6.7E-02 1.51E+03 0 3.13E-01 9.1E-01 3.2E-02 -9.84E+01
SM kg 2.07E+00 0 0 0 0 0 0 0 0
RSF MJ 0 0 0 0 0 0 0 0 0
NRSF MJ 0 0 0 0 0 0 0 0 0
FW m3 1.92E-01 3.57E-06 6.21E-04 7.75E-01 0 1.77E-06 7E-03 8.03E-06 -5.8E-02
PERE = Use of renewable primary energy excluding renewable primary energy resources used as raw materials; PERM = Use of renewable primary
energy resources used as raw materials; PERT = Total use of renewable primary energy resources; PENRE = Use of non-renewable primary energy
excluding non-renewable primary energy resources used as raw materials; PENRM = Use of non-renewable primary energy resources used as raw
materials; PENRT = Total use of non-renewable primary energy resources; SM = Use of secondary material; RSF = Use of renewable secondary fuels;
NRSF = Use of non-renewable secondary fuels; FW = Use of net fresh water
RESULTS OF THE LCA – WASTE CATEGORIES AND OUTPUT FLOWS according to EN 15804+A2:
1 piece SafeRoute
Parameter Unit A1-A3 A4 A5 B6 C1 C2 C3 C4 D
HWD kg 1.53E-05 6.12E-11 9.9E-11 6.26E-07 0 3.03E-11 2.31E-09 4.86E-10 -1.9E-06
NHWD kg 1.94E+00 6.45E-05 7E-03 1.07E+00 0 3.2E-05 1.33E-01 1.6E-01 -5.34E-01
RWD kg 1.4E-02 6.78E-07 3.53E-06 2.3E-01 0 3.36E-07 4.12E-05 3.63E-07 -7E-03
CRU kg 0 0 0 0 0 0 0 0 0
MFR kg 0 0 0 0 0 0 3.7E+00 0 0
MER kg 0 0 0 0 0 0 0 0 0
EEE MJ 0 0 3.22E-01 0 0 0 4.75E+00 0 0
EET MJ 0 0 5.84E-01 0 0 0 9.67E+00 0 0
5 Environmental Product Declaration - dormakaba - SafeRoute
HWD = Hazardous waste disposed; NHWD = Non-hazardous waste disposed; RWD = Radioactive waste disposed; CRU = Components for re-use;
MFR = Materials for recycling; MER = Materials for energy recovery; EEE = Exported electrical energy; EET = Exported thermal energy
RESULTS OF THE LCA – additional impact categories according to EN 15804+A2-optional:
1 piece SafeRoute
Parameter Unit A1-A3 A4 A5 B6 C1 C2 C3 C4 D
Disease
PM 1.26E-06 2.34E-10 3.3E-10 1.59E-06 0 1.16E-10 3.89E-09 2.16E-10 -4.28E-07
incidence
IR kBq U235 eq 1.74E+00 9.68E-05 5.46E-04 3.77E+01 0 4.8E-05 5E-03 3.73E-05 -1.1E+00
ETP-fw CTUe 1.46E+02 4.47E-01 3.2E-02 6.47E+02 0 2.21E-01 3.64E-01 1.8E-02 -3.69E+01
HTP-c CTUh 1.16E-07 8.41E-12 1.69E-12 1.79E-08 0 4.17E-12 2.82E-11 2.7E-12 1.02E-08
HTP-nc CTUh 9.75E-07 3.6E-10 7.3E-11 6.58E-07 0 1.78E-10 2.15E-09 2.97E-10 1.29E-06
SQP SQP 2.62E+02 2E-03 1.8E-02 4.82E+02 0 8.03E-04 2.64E-01 7E-03 -9.64E+00
PM = Potential incidence of disease due to PM emissions; IR = Potential Human exposure efficiency relative to U235; ETP-fw = Potential comparative
Toxic Unit for ecosystems; HTP-c = Potential comparative Toxic Unit for humans (cancerogenic); HTP-nc = Potential comparative Toxic Unit for humans
(not cancerogenic); SQP = Potential soil quality index
Disclaimer 1 – for the indicator “Potential Human exposure efficiency relative to U235”. This impact category deals mainly with the
eventual impact of low-dose ionizing radiation on human health of the nuclear fuel cycle. It does not consider effects due to possible
nuclear accidents, occupational exposure or radioactive waste disposal in underground facilities. Potential ionizing radiation from the
soil, radon and from some construction materials is also not measured by this indicator.
Disclaimer 2 – for the indicators “abiotic depletion potential for non-fossil resources”, “abiotic depletion potential for fossil resources”,
“water (user) deprivation potential, deprivation-weighted water consumption”, “potential comparative toxic unit for ecosystems”,
“potential comparative toxic unit for humans – cancerogenic”, “Potential comparative toxic unit for humans - not cancerogenic”,
“potential soil quality index”. The results of this environmental impact indicator shall be used with care as the uncertainties on these
results are high as there is limited experience with the indicator.
This EPD was created using a software tool.
References
ISO 14025 GaBi
DIN EN ISO 14025:2011-10, Environmental labels and Sphera Solutions GmbH Gabi Software System and Database
declarations — Type III environmental declarations — for Life Cycle Engineering 1992-2020 Version 10.0.0.71
Principles and procedures University of Stuttgart Leinfelden-Echterdingen
EN 15804 GaBi ts documentation
EN 15804+A2:2019+AC:2021, Sustainability of construction GaBi life cycle inventory data documentation (https://www.gabi-
works — Environmental Product Declarations — Core rules for software.com/support/gabi/gabidatabase- 2020-lci-
the product category of construction products documentation/)
EN 13637 LCA-tool dormakaba
DIN EN 13637:2015-12 Building hardware - Electrically LCA tool, version DHW. Tool No.: IBU-DOR-202104-LT1-EN
controlled exit systems for use on escape routes - Developed by Sphera Solutions GmbH
Requirements and test methods
PCR Part A
REACH PCR – Part A: Calculation Rules for the Life Cycle Assessment
Registration, Evaluation, Authorisation and Restriction of and Requirements on the Project Re-port according to EN
Chemicals (REACH), Regulation (EC) No 1907/2006 15804+A2:2019, Version 1.0, 2020, Institut Bauen und Umwelt
e.V., www.ibu-epd.com
2011/65/EU ROHS3 Directive
Directive 2011/65/EU of the European Parliament and of the PCR Part B
Council of 8 June 2011 on the restriction of the use of certain PCR – Part B: Requirements on the EPD for Building Hardware
hazardous substances in electrical and electronic equipment product, version 1.2, Institut Bauen und Umwelt e.V., www.ibu-
epd.com, 2017
Further References
IBU 2021
General Instructions for the EPD programme of Institut Bauen
und Umwelt e.V. Version 2.0, Berlin: Institut Bauen und Umwelt
e.V., 2021. www.ibu-epd.com
6 Environmental Product Declaration - dormakaba - SafeRoute
Publisher
Institut Bauen und Umwelt e.V. +49 (0)30 3087748- 0
Hegelplatz 1 info@ibu-epd.com
10117 Berlin www.ibu-epd.com
Germany
Programme holder
Institut Bauen und Umwelt e.V. +49 (0)30 3087748- 0
Hegelplatz 1 info@ibu-epd.com
10117 Berlin www.ibu-epd.com
Germany
Author of the Life Cycle Assessment
dormakaba International Holding GmbH +49 2333 793-0
DORMA Platz 1 info.de@dormakaba.com
58256 Ennepetal www.dormakaba.com
Germany
Owner of the Declaration
dormakaba International Holding GmbH +49 2333 793-0
DORMA Platz 1 info.de@dormakaba.com
58256 Ennepetal www.dormakaba.com
Germany
7 Environmental Product Declaration - dormakaba - SafeRoute
