ENVIRONMENTAL PRODUCT DECLARATION
as per ISO 14025 and EN 15804+A2
Owner of the Declaration Olam Agri - Congolaise Industrielle des Bois
Publisher Institut Bauen und Umwelt e.V. (IBU)
Programme holder Institut Bauen und Umwelt e.V. (IBU)
Declaration number EPD-CON-20230314-LT1-EN
Issue date 27.11.2023
Valid to 26.11.2028
Sapelli Kiln Dried Timber
Congolaise Industrielle Des Bois SA (CIB)
www.ibu-epd.com | https://epd-online.com
General Information
Congolaise Industrielle Des Bois SA (CIB) Sapelli Kiln Dried Timber
Programme holder Owner of the declaration
IBU – Institut Bauen und Umwelt e.V. Olam Agri - Congolaise Industrielle des Bois
Hegelplatz 1 Pokola BP 41
10117 Berlin BP 41 Ouesso
Germany (Others)
Declaration number Declared product / declared unit
EPD-CON-20230314-LT1-EN Sapelli kiln-dried lumber, per m3
This declaration is based on the product category rules: Scope:
Solid wood products, 01.08.2021 This Environmental Product Declaration refers to Sapelli wood that is
(PCR checked and approved by the SVR) harvested, sawn, air dried and kiln-dried by the Congolaise Industrielle des
Bois (CIB). CIB's forestry concessions and industrial site are located in the
Republic of the Congo, Sangha department (site of Pokola) and Likouala
Issue date department (site of Enyelle).
27.11.2023
CIB forests and production are 100% FSC certified.
This life cycle analysis is based on data from 2021.
Valid to
26.11.2028 CIB is fully owned by Olam Global Agri Pte. Ltd.
The owner of the declaration shall be liable for the underlying information
and evidence; the IBU shall not be liable with respect to manufacturer
information, life cycle assessment data and evidences.
The EPD was created according to the specifications of EN 15804+A2. In
the following, the standard will be simplified as EN 15804.
Verification
The standard EN 15804 serves as the core PCR
Independent verification of the declaration and data according to ISO
Dipl.-Ing. Hans Peters
14025:2011
(Chairman of Institut Bauen und Umwelt e.V.)
internally X externally
Florian Pronold Prof. Dr. Birgit Grahl,
(Managing Director Institut Bauen und Umwelt e.V.) (Independent verifier)
1 Environmental Product Declaration - Congolaise Industrielle Des Bois SA (CIB) - Sapelli Kiln Dried Timber
Product
Product description/Product definition
Constructional data
Sapelli kiln-dried lumber is produced according to the following
process: Name Value Unit
Wood types by trade names
Sapelli -
Trees are inventoried, counted, and harvested as per our forest acc. to Tropix
management plans. Wood moisture 12 %
Gross density acc. to Tropix 690 kg/m3
Logs are exported to CIB facilities in Pokola and Enyelle, sorted
Class 3 - moderately
by quality and sawn in one of CIB's sawmills according to the Risk class acc. to Tropix -
durable
customer requirements of lengths, thickness, width and quality.
Performance data of the product with respect to its
Lumber is stack on stickers and left on our site for air-drying for characteristics in accordance with the relevant technical
a period varying between 3 weeks to 6 months, depending on provision (no CE-marking).
the thickness.
Base materials/Ancillary materials
When wood has reached its fibre saturation point, it is taken The wood specie of this lumber is Sapelli (entandrophragma
into our kilns for a drying cycle varying between 3 days to 6 cylindricum).
weeks. Final moisture content depends on customer
requirements and usually varies from 8% to 16%. 1) This product contains substances listed in the candidate list
(date: 17.10.2023) exceeding 0.1 percentage by mass: no
After kilining, bundles are destacked, inspected, defects planks
are removed and final bundles are stacked, strapped and 2) This product contains other Carcinogenic, Mutagenic,
marked for export. Reprotoxic (CMR) substances in categories 1A or 1B which are
For the use and application of the product the respective not on the candidate list, exceeding 0.1 percentage by mass:
national provisions at the place of use apply, in Germany for no
example the building codes of the federal states and the
corresponding national specifications. 3) Biocide products were added to this construction product or it
has been treated with biocide products (this then concerns a
Application treated product as defined by the (EU) Ordinance on Biocide
Sapelli wood has multiple used: doors and windows frame, Products No. 528/2012): no
moulded products, furnitures, etc.
Reference service life
Technical Data Depending on how and where it is used (internal, external) and
Technical data on Sapelli wood can be found on the CIRAD's various conditions (weather, exposition to sun, rain, humidity),
Tropix database at the following link: Sapelli lumber is durable for several decades.
https://tropix.cirad.fr/FichiersComplementaires/EN/Africa/SAPELLI.pdf.
LCA: Calculation rules
site production via biomass power plant).
Declared Unit • The scenario for the transport of the product to the
The declaration refers to the declared unit of 1m³ of Sapelli Kiln construction site is declared in module A4.
Dried Timber. The density of the final product is 690kg/m³. • The treatment of packaging materials at installation is
Declared unit declared in module A5. Sapelli KD Timber is a pre-
product, the installation of such product is very variable.
Name Value Unit
The installation stage (e.g. installation process and
Declared unit 1 m3 potential auxiliaries) has been excluded from the scope
Gross density 690 kg/m3 of the study.
Wood moisture (upon delivery) 12 % • The end-of-life scenarios include, deconstruction (C1),
transportation to waste processing (C2), emissions and
Water content = 11%
energy requirements of combustion (C3). Benefits and
Moisture content = 12%
loads for the next system (e.g. electricity and thermal
energy, which result from energy recovery in modules
A5 and C3) are declared in module D.
• The CO2 incorporation in the product (from the
System boundary
sequestration in the wood) is considered. The C-balance
The type of EPD is cradle to gate with options, module C1-C4,
is closed by considering the biotic GHG emissions
and module D (A1-A3, C, D and additionnal modules A4 and
according to the incorporation on input side.
A5).
The data collected by the manufacturers is based on yearly
production amounts. The production data refers to the yearly
Considered product stages:
consumption in 2021.
• Production of raw materials (e.g. log extraction from the
forest), extraction of energy carriers, raw material Geographic Representativeness
transportation, manufacture of product and packaging Land or region, in which the declared product system is
materials are declared in modules A1-A3. Modules A1- manufactured, used or handled at the end of the product´s
A3 also include the generation and supply of energy (on lifespan: Global
2 Environmental Product Declaration - Congolaise Industrielle Des Bois SA (CIB) - Sapelli Kiln Dried Timber
the product-specific characteristics of performance, are taken
Comparability into account. Background dataset : GaBi ts software, CUP
Basically, a comparison or an evaluation of EPD data is only 2022.1.
possible if all the data sets to be compared were created
according to EN 15804 and the building context, respectively
LCA: Scenarios and additional technical information
Packaging material:
Characteristic product properties of biogenic carbon Plastic film : 0,20 kg/m³
The product and packaging material (wooden wedges) contains Plastic straps : 0,84 kg/m³
biogenic carbon. The following biogenic carbon content is Steel straps : 0,11 kg/m³
assumed : Steel buckles: 0,11 kg/m³
- 0,484kg C /kg of hardwood wood (dry) Wooden wedges: 3,60 kg/m³
- 0,5kg C /kg of wooden wedges (dry)
Information on describing the biogenic Carbon Content at
factury gate End of life (C1-C4)
Name ValueUnit The end-of-life scenarios are as follows:
kg
Biogenic carbon content in product 298
C C1 – Dismantling / Demolition: Sapelli KD Timber is a pre-
product and the deconstruction methods of the product cannot
Biogenic carbon content in accompanying kg
1.48 be foreseen. The deconstruction is therefor omitted from the
packaging C
scope of the EPD. As module C1 is a mandatory module, it is
Note: 1 kg of biogenic carbon is equivalent to 44/12 kg of CO 2. included in the EPD but not declared, according to the PCR-A.
C2 – Transport to treatment/disposal site: Average transport
The following technical scenario information is required for the distance from the demolition site to waste treatment is assumed
declared modules. as 50 km to thermal treatment.
Transport to the building site (A4)
C3 – Waste treatment: The Sapelli Kiln Dired Timber is 100 %
The transportation of the Sapelli KD Timber from the
combusted with energy recovery.
manufacturing plant in Pokola, Republic of Congo to the
construction site in Europe is considered.
C4 – Disposal: No disposal scenario.
Name Value Unit
Name Value Unit
Litres of fuel 1.52 l/100km
Collected separately waste type 690 kg
Transport distance (via truck) 1304 km
Energy recovery 690 kg
Capacity utilisation (including empty runs) 61 %
Gross density of products transported 690 kg/m3
Reuse, recovery and/or recycling potentials (D), relevant
Transport distance (via ocean ship) 9260 km scenario information
Installation into the building (A5)
For the thermal and electrical energy generated in module A5
Module A5 includes the waste processing up to the end-of-
due to thermal treatment of packaging and C3 for the
waste state or disposal of packaging materials during the
incineration of the product, avoided burdens have been
construction process stage. The installation stage (e.g.
calculated by the inversion of electricity grid mix and thermal
installation process and potential auxiliaries) has been
energy from natural gas, using European datasets. Material
excluded from the scope of the study.
benefits are also given for the recycling of metal packaging
Name ValueUnit materials (steel buckles and steel straps).
Output substances following waste treatment on
4.85 kg
site
3 Environmental Product Declaration - Congolaise Industrielle Des Bois SA (CIB) - Sapelli Kiln Dried Timber
LCA: Results
The following tables display the environmentally relevant results according to EN 15804+A2 (EF 3.0) for 1 m³ of Sapelli KD Timber.
Please be aware, the module A5 only considers the disposal of packaging material, and do not the complete installation scenario
because the declared product is a pre-product and installation is unknown.
DESCRIPTION OF THE SYSTEM BOUNDARY (X = INCLUDED IN LCA; MND = MODULE OR INDICATOR NOT DECLARED; MNR
= MODULE NOT RELEVANT)
Benefits and
Construction loads beyond
Product stage Use stage End of life stage
process stage the system
boundaries
la ire ta m w a Ry lp p u s tro p s n a rT g n iru tc a fu n a M e h t m o rf tro p s n a rTe tis e h t o t e ta g y lb m e s s A e s U e c n a n e tn ia M ria p e R tn e m e c a lp e R tn e m h s ib ru fe R y g re n e la n o ita re p Oe s u re ta w la n o ita re p Oe s u n o itc u rts n o c -e Dn o itilo m e d tro p s n a rT g n is s e c o rp e ts a W la s o p s iD -e s u e R-y re v o c e R-g n ilc y c e Rla itn e to p
A1 A2 A3 A4 A5 B1 B2 B3 B4 B5 B6 B7 C1 C2 C3 C4 D
X X X X X MND MND MNR MNR MNR MND MND X X X X X
RESULTS OF THE LCA - ENVIRONMENTAL IMPACT according to EN 15804+A2: 1 m³ Sapelli KD Timber
Parameter Unit A1-A3 A4 A5 C1 C2 C3 C4 D
GWP-total kg CO 2 eq -9.08E+02 1.16E+02 8.1E+00 ND 2.42E+00 1.11E+03 0 -3.63E+02
GWP-fossil kg CO 2 eq 1.79E+02 1.13E+02 2.7E+00 ND 2.3E+00 1.88E+01 0 -3.61E+02
GWP-biogenic kg CO 2 eq -1.09E+03 2.65E+00 5.41E+00 ND 1.08E-01 1.09E+03 0 -1.85E+00
GWP-luluc kg CO 2 eq 7.43E-01 6.64E-04 4.14E-05 ND 1.55E-02 2.71E-03 0 -3.97E-02
ODP kg CFC11 eq 2.31E-11 4.16E-13 8.73E-13 ND 2.26E-13 1.25E-10 0 -2.44E-09
AP mol H+ eq 8.6E+00 2.05E+00 1.11E-03 ND 2.58E-03 1.64E-01 0 -4.76E-01
EP-freshwater kg P eq 1.79E-04 2.14E-05 2.19E-07 ND 8.23E-06 2.82E-05 0 -4.97E-04
EP-marine kg N eq 2.64E+00 5.39E-01 3.46E-04 ND 8.34E-04 5.3E-02 0 -1.29E-01
EP-terrestrial mol N eq 4.06E+01 5.91E+00 5.22E-03 ND 9.98E-03 7.65E-01 0 -1.38E+00
kg NMVOC
POCP 3.06E+01 1.52E+00 9.54E-04 ND 2.22E-03 1.44E-01 0 -3.61E-01
eq
ADPE kg Sb eq 7.28E-06 1.04E-06 2.22E-08 ND 2.32E-07 2.81E-06 0 -5.53E-05
ADPF MJ 1.75E+03 1.54E+03 2.38E+00 ND 3.02E+01 2.82E+02 0 -6.14E+03
m3 world eq
WDP 9.22E+00 1.39E-01 8.12E-01 ND 2.58E-02 1.16E+02 0 -3.85E+01
deprived
GWP = Global warming potential; ODP = Depletion potential of the stratospheric ozone layer; AP = Acidification potential of land and water; EP =
Eutrophication potential; POCP = Formation potential of tropospheric ozone photochemical oxidants; ADPE = Abiotic depletion potential for non-fossil
resources; ADPF = Abiotic depletion potential for fossil resources; WDP = Water (user) deprivation potential)
RESULTS OF THE LCA - INDICATORS TO DESCRIBE RESOURCE USE according to EN 15804+A2: 1 m³ Sapelli KD Timber
Parameter Unit A1-A3 A4 A5 C1 C2 C3 C4 D
PERE MJ 3.16E+04 8.74E-01 5.36E+01 ND 2.1E+00 1.12E+04 0 -1.69E+03
PERM MJ 1.11E+04 0 -5.31E+01 ND 0 -1.11E+04 0 0
PERT MJ 4.27E+04 8.74E-01 5.09E-01 ND 2.1E+00 8.2E+01 0 -1.69E+03
PENRE MJ 1.7E+03 1.54E+03 5.02E+01 ND 3.03E+01 2.82E+02 0 -6.14E+03
PENRM MJ 4.78E+01 0 -4.78E+01 ND 0 0 0 0
PENRT MJ 1.75E+03 1.54E+03 2.38E+00 ND 3.03E+01 2.82E+02 0 -6.14E+03
SM kg 2.79E-02 0 0 ND 0 0 0 0
RSF MJ 0 0 0 ND 0 0 0 0
NRSF MJ 0 0 0 ND 0 0 0 0
FW m3 2.39E-01 4.54E-03 1.91E-02 ND 2.42E-03 2.74E+00 0 -1.62E+00
PERE = Use of renewable primary energy excluding renewable primary energy resources used as raw materials; PERM = Use of renewable primary
energy resources used as raw materials; PERT = Total use of renewable primary energy resources; PENRE = Use of non-renewable primary energy
excluding non-renewable primary energy resources used as raw materials; PENRM = Use of non-renewable primary energy resources used as raw
materials; PENRT = Total use of non-renewable primary energy resources; SM = Use of secondary material; RSF = Use of renewable secondary fuels;
NRSF = Use of non-renewable secondary fuels; FW = Use of net fresh water
RESULTS OF THE LCA – WASTE CATEGORIES AND OUTPUT FLOWS according to EN 15804+A2:
1 m³ Sapelli KD Timber
Parameter Unit A1-A3 A4 A5 C1 C2 C3 C4 D
HWD kg 1.1E-08 3.79E-10 1.9E-10 ND 1.61E-10 2.67E-08 0 -8.31E-07
NHWD kg 4.41E+00 9.62E-03 2.73E-01 ND 4.94E-03 8.04E+00 0 -3.06E+00
RWD kg 3.63E-03 6.3E-05 1.07E-04 ND 5.63E-05 2.19E-02 0 -4.84E-01
CRU kg 0 0 0 ND 0 0 0 0
MFR kg 2.34E+02 0 1.92E-01 ND 0 0 0 0
MER kg 0 0 0 ND 0 0 0 0
4 Environmental Product Declaration - Congolaise Industrielle Des Bois SA (CIB) - Sapelli Kiln Dried Timber
EEE MJ 0 0 1.26E+01 ND 0 1.61E+03 0 0
EET MJ 0 0 2.26E+01 ND 0 2.89E+03 0 0
HWD = Hazardous waste disposed; NHWD = Non-hazardous waste disposed; RWD = Radioactive waste disposed; CRU = Components for re-use;
MFR = Materials for recycling; MER = Materials for energy recovery; EEE = Exported electrical energy; EET = Exported thermal energy
RESULTS OF THE LCA – additional impact categories according to EN 15804+A2-optional:
1 m³ Sapelli KD Timber
Parameter Unit A1-A3 A4 A5 C1 C2 C3 C4 D
Disease
PM 2.38E-03 3.43E-05 7.84E-09 ND 1.77E-08 8.27E-07 0 -3.95E-06
incidence
IR kBq U235 eq 5.52E-01 5.38E-03 1.65E-02 ND 8.51E-03 3.63E+00 0 -8.19E+01
ETP-fw CTUe 2.4E+03 4.27E+02 1.39E+00 ND 2.14E+01 1.24E+02 0 -1.35E+03
HTP-c CTUh 8.27E-06 7.01E-09 7.62E-11 ND 4.42E-10 7.59E-09 0 -6.21E-08
HTP-nc CTUh 6.06E-05 2.6E-07 5.24E-09 ND 2.39E-08 2.66E-07 0 -2.38E-06
SQP SQP 5.37E+05 6.17E-01 5.81E-01 ND 1.28E+01 8.69E+01 0 -1.1E+03
PM = Potential incidence of disease due to PM emissions; IR = Potential Human exposure efficiency relative to U235; ETP-fw = Potential comparative
Toxic Unit for ecosystems; HTP-c = Potential comparative Toxic Unit for humans (cancerogenic); HTP-nc = Potential comparative Toxic Unit for humans
(not cancerogenic); SQP = Potential soil quality index
Disclaimer 1 – for the indicator 'Potential Human exposure efficiency relative to U235'.This impact category deals mainly with the
eventual impact of low dose ionizing radiation on human health of the nuclear fuel cycle. It does not consider effects due to possible
nuclear accidents, occupational exposure or radioactive waste disposal in underground facilities. Potential ionizing radiation from the
soil, radon and from some construction materials is also not measured by this indicator.
Disclaimer 2 – for the indicators 'abiotic depletion potential for non-fossil resources', 'abiotic depletion potential for fossil resources',
'water (user) deprivation potential, deprivation-weighted water consumption', 'potential comparative toxic unit for ecosystems', 'potential
comparative toxic unit for humans – cancerogenic', 'Potential comparative toxic unit for humans - not cancerogenic', 'potential soil
quality index'. The results of this environmental impact indicator shall be used with care as the uncertainties on these results are high
as there is limited experience with the indicator. This EPD was created using a software tool.
References
Standards University of Stuttgart, program version GaBi 10; database
version 2022.1
EN 15804
EN 15804:2012+A2:2019+AC:2021, Sustainability GaBi documentation
ofconstruction works — Environmental Product Declarations — GaBi dataset documentation for the software system and
Core rules for the product category of construction products. databases, LBP, University of Stuttgart and Sphera Solutions
GmbH, Leinfelden-Echterdingen, 2021.
ISO 14025 (http://www.gabi-software.com/support/gabi/gabi[1]database-
EN ISO 14025:2011, Environmental labels anddeclarations — 2021-lci-documentation/)
Type III environmental declarations — Principles and
procedures. PCR Part A
PCR - Part A: Calculation rules for the Life Cycle Assessment
Further References and Requirements on the Background Report, version 1.3 from
08.2022, Institut Bauen und Umwelt e.V., www.bau-umwelt.com
IBU 2021
Institut Bauen und Umwelt e.V.: General Instructions for the PCR Part B
EPD programme of Institut Bauen und Umwelt e.V., Version Part B: Requirements on the EPD for Solid wood product,
2.0, Berlin: Institut Bauen und Umwelt e.V., 2021 www.ibu- version from 08.2021
epd.com
TROPIX
GaBi Fiche de l'essence Sapelli, TROPIX database, available at:
GaBi Software System and Database for Life https://tropix.cirad.fr/FichiersComplementaires/EN/Africa/SAPELLI.pdf
CycleEngineering, 1992-2021, Sphera Solutions GmbH,
Leinfelden-Echterdingen, with acknowledgement of LBP
5 Environmental Product Declaration - Congolaise Industrielle Des Bois SA (CIB) - Sapelli Kiln Dried Timber
Publisher
Institut Bauen und Umwelt e.V. +49 (0)30 3087748- 0
Hegelplatz 1 info@ibu-epd.com
10117 Berlin www.ibu-epd.com
Germany
Programme holder
Institut Bauen und Umwelt e.V. +49 (0)30 3087748- 0
Hegelplatz 1 info@ibu-epd.com
10117 Berlin www.ibu-epd.com
Germany
Author of the Life Cycle Assessment
Sphera Solutions GmbH +49 711 341817-0
Hauptstraße 111- 113 info@sphera.com
70771 Leinfelden-Echterdingen www.sphera.com
Germany
Owner of the Declaration
Olam Agri - Congolaise Industrielle des Bois +41612053944
Pokola BP 41 crs.congo@olamagri.com
BP 41 Ouesso www.olamagri.com
(Others)
6 Environmental Product Declaration - Congolaise Industrielle Des Bois SA (CIB) - Sapelli Kiln Dried Timber
