ENVIRONMENTAL PRODUCT DECLARATION
as per ISO 14025 and EN 15804+A1
Owner of the Declaration Etex Building Performance International
Programme holder Institut Bauen und Umwelt e.V. (IBU)
Publisher Institut Bauen und Umwelt e.V. (IBU)
Declaration number EPD-ETX-20200007-IBA1-EN
Issue date 08.01.2020
Valid to 07.01.2025
MASTERIMPACT®-RH
Fibre cement drywall panels
Etex Building Performance International
www.ibu-epd.com | https://epd-online.com
Umwelt Produktdeklaration Name des Herstellers – Name des Produkts
1. General Information
Etex Building Performance International MASTERIMPACT®-RH Drywall Panel
Programme holder Owner of the declaration
IBU – Institut Bauen und Umwelt e.V. Etex Building Performance International
Panoramastr. 1 500 rue Marcel Demonque
10178 Berlin 84915 Avignon Cedex 9
Germany FRANCE
Declaration number Declared product / declared unit
EPD-ETX-20200007-IBA1-EN 1m² MASTERIMPACT®-RH
This declaration is based on the product Scope:
category rules: The Environmental Product Declaration includes the
Fibre cement / Fibre concrete, 07.2014 environmental parameters for the MASTERIMPACT®-
(PCR checked and approved by the SVR) RH drywall panels produced by Etex Building
performance International. The result of the life cycle
assessment provided in this EPD is based on a
Issue date
thickness of 9mm.
08.01.2020
This document refers to the structural panels
manufactured in the Kapelle-op-den-Bos plant
Valid to
(Belgium). The production data used refers to the
07.01.2025 production year 2016. Based on plausible, transparent
and comprehensible basic data, the Life Cycle
Assessment fully represents the Etex products in
question.
In an annex to this EPD the LCA results for additional
thicknesses (6 mm and 12 mm) are declared.
The owner of the declaration shall be liable for the
underlying information and evidence; the IBU shall not
be liable with respect to manufacturer information, life
cycle assessment data and evidences.
The EPD was created according to the specifications
of EN 15804+A1. In the following, the standard will be
simplified as EN 15804.
Verification
The standard EN 15804 serves as the core PCR
Independent verification of the declaration and data
according to ISO 14025:2010
Dipl. Ing. Hans Peters internally x externally
(chairman of Institut Bauen und Umwelt e.V.)
Dr. Alexander Röder Dipl. Natw. ETH Sascha Iqbal
(Managing Director Institut Bauen und Umwelt e.V.)) (Independent verifier appointed by SVR)
2. Product
2.1 Product description/Product definition CE Declaration of Conformity in accordance with the
This Environmental Product Declaration refers to large- specifications outlined in Annex ZA to /EN 12467/.
format structural panels comprising cellulose- European Technical Assesment /ETA 06/0207/, 2018-
reinforced fibre-cement panels. The products under 06-25.
review involve smooth panels made from steam-
hardened fibre cement. External monitoring of the products with general
technical approval by the Material Testing Institute of
For the placing on the market of the product in the the state of Brandenburg/Berlin and the German
European Union / European Free Trade Association Federal Institute for Materials Research and Testing
(EFTA) (with the exception of Switzerland) the (/BAM/).
/Construction Products Regulation/ applies. The
product needs a declaration of performance taking into For the application and the use, the respective national
consideration /EN 12467/: Fibre-cement flat sheets - provisions apply.
Product specification and test methods.
2 Environmental Product Declaration ETEX – MASTERIMPACT®-RH Fibre-Cement Drywall Panels
2.2 Application widely used asbestos cement products manufactured
MASTERIMPACT®-RH is a building board for interior before that time.
areas exposed to high levels of humidity. It serves as a Information that product does not contain substances
backer board for tiles and moisture-resistant top coat listed in the Candidate List of substances of very high
systems. concern (/REACH Regulation/) exceeding 0.1%:
This product contains substances listed in the
2.3 Technical Data candidate list (date: 15.01.2019) exceeding 0.1 % by
Sound insulation: mass: no
A sound insulation value of Rw = 54 dB is achieved in
a reinforced steel partition wall system with metal This product contains other carcinogenic, mutagenic
profiles 50 mm in depth, cladding on both sides with 2 and toxic for reproduction (CMR) substances in
x 12 mm MASTERIMPACT®-RH and the reinforced categories 1A or 1B which are not on the candidate
steel partition wall lined with 40 mm mineral wool infill. list, exceeding 0.1 % by mass: no
Standard-related tests for CE marking via type testing
in accordance with /EN 12467/. Biocide products were added to this construction
product or it has been treated with biocide products
Constructional data (this then concerns a treated product as defined by the
Name Value Unit (EU) /Ordinance on Biocide Products/):
Gross density dry, mean, +/- 10% 1180 kg/m3 no
Compressive strength 38 N/mm2
Modulus of elasticity perpendicular >7.5 N/mm2 2.6 Manufacture
Modulus of elasticity parallel >8.5 N/mm² Large-format panels made of fibre cement are
Flexural strength perpendicular >10.4 N/mm2 manufactured mainly in accordance with an automated
Flexural strength parallel >16.9 N/mm² winding process. The raw materials are treated with
Tensile strength 6.3 N/mm2 water to form a homogeneous mixture. Rotating screen
cylinders are immersed in this fibre cement pulp which
84 (wet)
Water vapour diffusion resistance drains the mixture outwards.
- 143 -
factor The screen surface is coated with a thin fibre cement
(dry)
film which is conveyed onto an infinite transport belt
Moisture content at 23 °C, 80%
6 M.-% from where it reaches a format roller to which an
humidity
increasingly thick layer of fibre cement is applied. Once
Coefficient of thermal expansion <6.5 10-6K-1
the requisite material thickness has been achieved, the
Swelling (air-dry to water-saturated) 7 mm/m
still moist and malleable fibre cement layer (fibre
similar to
cement fleece) is unravelled and detached from the
Chemical resistance concrete -
format roller.
C35/C45
The fibre cement fleece is cut to length and any
similar to
leftovers are returned to the production process with
Ageing resistance concrete -
the result that no waste is incurred. The panels are
C35/C45
then set aside for binding before stacking on pallets
up to
Permanent temperature resistance °C and steam-hardened in an autoclave for approx. 2
100
hours. The setting time lasts approx. 3 days.
Thermal conductivity 0.19 W/(mK)
Quality Management
The production facilities are TÜV-certified in
Performance data of the product in accordance with accordance with /ISO 9001/.
the declaration of performance with respect to its
essential characteristics according to /EN 12467/. 2.7 Environment and health during
manufacturing
2.4 Delivery status During the entire manufacturing process, there are no
The MASTERIMPACT®-RH is delivered with a other health protection measures extending beyond
maximum size of 3.100 mm x 1.500 mm in three the legally specified industrial protection measures for
strenghts of 6 mm, 9 mm and 12 mm and with a commercial enterprises.
smooth surface.
 Air: Any dust incurred is collected in filter
systems and partially re-used. Emissions are
2.5 Base materials/Ancillary materials
significantly lower than the limit values
Base materials in % mass (dry mass)
specified by the TA Air.
 25-45% Portland cement to /EN 197-1/, (CEM  Water/Soil: Water incurred during
I 32.5 R and 42.5 R) (binding agent) manufacturing and plant cleaning is treated
 25-45% Quartz sand, mineral aggregates mechanically in waste water treatment
 1-15% Wollastonite systems on the plant site and re-used in the
 1-10% Cellulose fibres production process.
 1-10% Mica  Noise: The noise emissions into the
 1-10% Aluminium hydroxide environment by production equipment fall
short of the permissible limit values.
and water for mixing the cement: 0.24 m³/t fibre
cement. The production facilities are certified in accordance
Cellulose-reinforced fibre cement products were with /ISO 14001/ and /OHSAS 18001/.
introduced in 1980s as a safe replacement for the
3 Environmental Product Declaration ETEX – MASTERIMPACT®-RH Fibre-Cement Drywall Panels
2.8 Product processing/Installation Building materials classification to /EN 13501-1/ A2,s1-
Special low-dust equipment such as slow-running, d0, i.e. limited combustibility in accordance with Part A
carbide-tipped splitting saws or cutting burs are of the Building Rules List.
available for processing. Drill holes can be made using
standard high-speed steel twist (HSS) drills. Additional Development of smoke/smoke density: smoke
products required for installing the products under development caused by burning the products in
review include: wood or metal substructures including question (coating) is very low.
the requisite anchoring and joining components as well
as securing parts (screws, nails, staples). When Combustion gases: the results in line with testing to
selecting any requisite constructive products, please /DIN 53436/ indicate that the gaseous emissions
ensure that they do not have a negative influence on incurred when burning the panels in question are free
the designated function of the construction products of sulphur and chlorine compounds. The concentration
referred to. of released hydrogen cyanide (HCN) is within a normal
The set of rules laid out by the employers' liability framework.
insurance associations shall apply.
When processing the products under review, Changing the system condition (burning dripping/falling
conventional industrial protection measures must be material): When surrounding construction materials are
observed in accordance with information supplied by burned, the cellulose fibres bound in the cement
the manufacturer. Please note that dust generated gradually lose their strength: This does not represent
during processing can have an alkaline reaction (pH any explosive potential with the result that fibre cement
value: >10). does not pose a risk in the event of a fire. Burning
According to the present state of knowledge, hazards dripping/falling hydrophobic treatment or fibre cement
for water, air and soil can not arise when fibre cement do not occur.
is processed as designated.
Water
2.9 Packaging No ingredients are washed out which could be
Cardboard boxes, wooden pallets and steel bands are hazardous to water (see also “Eluate analysis” in
used as packaging materials. The wooden pallets can Evidence). The pH value is alkaline (pH ≥ 10).
be returned by the customer and reused several times.
Mechanical destruction
Not of relevance
2.10 Condition of use
Hydration of the cement and water mixture forms 2.14 Re-use phase
hardened cement paste (calcium silicate hydrate) with De-construction: depending on the mounting system,
embedded fibres and fillers as well as micro air pores. the structural panels can be removed non-destructively
The fibre-cement products comprise approx. 6% water by unscrewing or opening the studs.
(equilibrium moisture) and a proportion by volume of
approx. 30% air (contained in the micro-pores). Re-use / further use: if undamaged, de-constructed
After the binding agent has set and when used as panels can be re-used as backer board or as
designated, fibre cement products can be used for foundation protection.
practically any applications. No maintenance or repair
is required over the service life of the boards. Re-use / Further use: when separated by type, fibre-
cement products referred to can be re-ground and re-
2.11 Environment and health during use used as additives in the manufacture of fibre cement
Environmental protection: According to the present (material recycling). When sorted by type, the fibre-
state of knowledge, hazards for water, air and soil cement products in question are also suitable for
cannot arise when the products under review are further use as a filler and loose material in civil
processed as designated (see chapter 7). engineering, especially in road construction or for
noise barriers (material recycling).
Health protection: When the construction products
are used as designated, no health hazards are known 2.15 Disposal
in connection with the base materials used and the Within the production process, most of the generated
performance thereof in the condition of use (see waste is immediately re-used within the process.
chapter 7). When after end-of-life re-using or recycling the boards
as described in the previous paragraph is not practical,
2.12 Reference service life the boards can be disposed to landfill class II.
When used in partition walls, the service life of The waste code in accordance with the /European
MASTERIMPACT®-RH is comparable with the Waste Index/ is 170904.
reference service life (RSL) of plasterboard.
The service life according to the "Bundesinstitut für 2.16 Further information
Bau-, Stadt- und Raumforschung" (/BBSR/) table is Further information is available on the following
indicated to be > 50 years. website: www.promat.be.
2.13 Extraordinary effects
Fire
Building materials class A2 as per /DIN 4102-1/, i.e.
limited combustibility.
4 Environmental Product Declaration ETEX – MASTERIMPACT®-RH Fibre-Cement Drywall Panels
3. LCA: Calculation rules
3.1 Declared Unit 3.4 Cut-off criteria
This declaration refers to the production of 1m2 All available data from production processes were
MASTERIMPACT®-RH (9mm, grammage 11.7 kg/m²) considered, i.e., all pre-products used, thermal energy
manufactured in Kapelle-op-den-Bos, Belgium. and electric power consumption as well as waste
management processes using best available life cycle
Declared unit inventory (LCI) datasets. This includes input flows with
Name Value Unit a contribution of less than 1% of mass or energy.
Declared unit 1 m² Production of capital equipment, facilities and
Gross density * 1290 kg/m3 infrastructure required for manufacture are outside the
Conversion factor to 1 t 0,0129 scope of this assessment.
* within range of 1180 kg/m³ +- 10%
3.5 Background data
The /GaBi ts software/ was used to model the product
3.2 System boundary life cycle. The basic data in the GaBi database is
Type of EPD: Cradle-to-gate with options. applied for energy, transportation, auxiliary products
The following life cycle stages and modules are and preliminary products. The software was revised in
included: 2018.
MASTERIMPACT®-RH is produced in Belgium.
Production stage (A1-A3): Belgian datasets were used for the grid mixes. For
 transportation and manufacturing of pre- other processes for which no Belgian datasets were
available, European average datasets were used (EU-
products to the manufacturing site
28).
 energy consumption and use of auxiliary
materials during production
3.6 Data quality
 disposal of production wastes The overall data quality and quality of the data
 production of packaging collection can be described as good. All relevant flows
were considered. Methodological choices are
consistent throughout the model.
Construction stage (A4-A5):
 transportation of product to the construction
3.7 Period under review
site Etex provided production data based on an annual
 energy consumption during the installation of average of the year 2016.
products
3.8 Allocation
 production of fixing- and finishing material
Production data refer to the declared product allocated
 disposal of installation wastes including
from the overall production volume (m2 virtually
emissions of biogenic CO 2 from cellulose normalised to 5 mm thickness) in Kapelle-op-den-Bos,
 disposal/incineration of packaging materials Belgium.
(potential benefits from energy substitution Specific information on allocation within the
within the incineration process are declared in background data is given in the /GaBi documentation/
(http://www.gabi-
module D) including emissions of biogenic
software.com/international/support/gabi/gabi-database-
CO from renewable packaging materials
2 2018-lci-documentation/).
Use stage (B1-B7): 3.9 Comparability
 efforts for the use of the product, Basically, a comparison or an evaluation of EPD data
maintenance and operational efforts is only possible if all the data sets to be compared
were created according to EN 15804 and the building
context, respectively the product-specific
End-of-life stage (C1-C4): characteristics of performance, are taken into account.
 energy consumption for de-construction and
demolition GaBi ts serves as background database for the
 transportation to disposal calculation of the life cycle assessment /GaBi ts
software/
 waste processing and landfilling of product
3.3 Estimates and assumptions .
No estimations or assumptions were made for the
production stage. Information on assumptions for the
scenarios in the life cycle of the product are described
in chapter 4.
5 Environmental Product Declaration ETEX – MASTERIMPACT®-RH Fibre-Cement Drywall Panels
4. LCA: Scenarios and additional technical information
Transport to the building site (A4)
Name Value Unit
Transport distance 600 km
Capacity utilisation (including empty
61 %
runs)
Installation into the building (A5)
Name Value Unit
Auxiliary Steel screws 0.128 kg
0.00016
Water consumption m3
1
Other resources : Powder mix finisher 0.35 kg
Electricity consumption 0.02 kWh
Material loss 0.35 kg
Dust in the air * 0 kg
VOC in the air 0 kg
* See chapter 2.8 for details regarding prevention of
dust emissions.
Use or application of the installed product (B1) see
section 2.11 "Use"
No efforts and releases of substances occur during the
normal (i.e. anticipated) use phase.
Maintenance (B2)
No efforts occur during maintenance.
Name Value Unit
Water consumption 0 m3
Auxiliary 0 kg
Other resources 0 kg
Electricity consumption 0 kWh
Other energy carriers 0 MJ
Waste materials resulting from
0 kg
maintenance
Operational energy use (B6) and Operational water
use (B7)
No efforts occur in modules B6 and B7. m2
Name Value Unit
Water consumption 0 m3
Electricity consumption 0 kWh
Other energy carriers 0 MJ
End of life (C1-C4)
Name Value Unit
Collected as mixed construction waste
12.2 kg
(incl. finisher and screws)
Recycling 0.1 kg
Landfilling 12.1 kg
6 Environmental Product Declaration ETEX – MASTERIMPACT®-RH Fibre-Cement Drywall Panels
5. LCA: Results
DESCRIPTION OF THE SYSTEM BOUNDARY (X = INCLUDED IN LCA; MND = MODULE NOT DECLARED;
MNR = MODULE NOT RELEVANT)
BENEFITS AND
CONSTRUCTI LOADS
PRODUCT STAGE ON PROCESS USE STAGE END OF LIFE STAGE BEYOND THE
STAGE SYSTEM
BOUNDARIES
7 Environmental Product Declaration ETEX – MASTERIMPACT®-RH Fibre-Cement Drywall Panels
lairetam
waR
ylppus tropsnarT
gnirutcafunaM
eht
morf
tropsnarT
etis
eht
ot
etag
ylbmessA esU
ecnanetniaM
riapeR
tnemecalpeR tnemhsibrufeR
ygrene
lanoitarepO esu
retaw
lanoitarepO esu
noitcurtsnoc-eD
noitilomed tropsnarT
gnissecorp
etsaW
lasopsiD -esueR -yrevoceR -gnilcyceR laitnetop
A1 A2 A3 A4 A5 B1 B2 B3 B4 B5 B6 B7 C1 C2 C3 C4 D
X X X X X X X MNR MNR MNR X X X X X X X
RESULTS OF THE LCA - ENVIRONMENTAL IMPACT according to EN 15804+A1: 1 m² MASTERIMPACT®-
RH (9 mm)
Parameter Unit A1-A3 A4 A5 B1 B2 B6 B7 C1 C2 C3 C4 D
GWP [kg CO2-Eq.] 5.78E+0 4.44E-1 9.73E-1 0.00E+0 0.00E+0 0.00E+0 0.00E+0 8.61E-3 3.83E-2 0.00E+0 1.56E+0 -1.96E-1
ODP [kg CFC11-Eq.] 4.73E-12 1.21E-14 7.15E-11 0.00E+0 0.00E+0 0.00E+0 0.00E+0 3.83E-14 1.04E-15 0.00E+0 6.25E-14 3.85E-14
AP [kg SO2-Eq.] 1.51E-2 1.03E-3 2.32E-3 0.00E+0 0.00E+0 0.00E+0 0.00E+0 2.44E-5 8.87E-5 0.00E+0 1.39E-3 -4.72E-4
EP [kg (PO4)3--Eq.] 2.29E-3 2.62E-4 3.48E-4 0.00E+0 0.00E+0 0.00E+0 0.00E+0 2.29E-6 2.26E-5 0.00E+0 2.18E-3 -4.04E-5
POCP [kg ethene-Eq.] 1.26E-3 -3.49E-4 2.64E-4 0.00E+0 0.00E+0 0.00E+0 0.00E+0 1.53E-6 -3.01E-5 0.00E+0 4.25E-4 -6.06E-5
ADPE [kg Sb-Eq.] 6.29E-6 3.63E-8 2.46E-5 0.00E+0 0.00E+0 0.00E+0 0.00E+0 4.57E-9 3.13E-9 0.00E+0 8.54E-8 2.02E-8
ADPF [MJ] 5.92E+1 6.01E+0 8.40E+0 0.00E+0 0.00E+0 0.00E+0 0.00E+0 9.16E-2 5.19E-1 0.00E+0 3.48E+0 -1.55E+0
GWP = Global warming potential; ODP = Depletion potential of the stratospheric ozone layer; AP = Acidification potential of land and water; EP =
Caption Eutrophication potential; POCP = Formation potential of tropospheric ozone photochemical oxidants; ADPE = Abiotic depletion potential for non-
fossil resources; ADPF = Abiotic depletion potential for fossil resources
RESULTS OF THE LCA - RESOURCE USE according to EN 15804+A1: 1 m² MASTERIMPACT®-RH (9 mm)
Parameter Unit A1-A3 A4 A5 B1 B2 B6 B7 C1 C2 C3 C4 D
PERE [MJ] 1.80E+1 3.33E-1 2.52E+0 0.00E+0 0.00E+0 0.00E+0 0.00E+0 5.91E-2 2.87E-2 0.00E+0 3.84E-1 1.42E-1
PERM [MJ] 1.00E+1 0.00E+0 0.00E+0 0.00E+0 0.00E+0 0.00E+0 0.00E+0 0.00E+0 0.00E+0 0.00E+0 0.00E+0 0.00E+0
PERT [MJ] 2.80E+1 3.33E-1 2.52E+0 0.00E+0 0.00E+0 0.00E+0 0.00E+0 5.91E-2 2.87E-2 0.00E+0 3.84E-1 1.42E-1
PENRE [MJ] 6.87E+1 6.04E+0 9.52E+0 0.00E+0 0.00E+0 0.00E+0 0.00E+0 1.57E-1 5.21E-1 0.00E+0 3.61E+0 -1.46E+0
PENRM [MJ] 0.00E+0 0.00E+0 0.00E+0 0.00E+0 0.00E+0 0.00E+0 0.00E+0 0.00E+0 0.00E+0 0.00E+0 0.00E+0 0.00E+0
PENRT [MJ] 6.87E+1 6.04E+0 9.52E+0 0.00E+0 0.00E+0 0.00E+0 0.00E+0 1.57E-1 5.21E-1 0.00E+0 3.61E+0 -1.46E+0
SM [kg] 3.07E-1 0.00E+0 9.19E-3 0.00E+0 0.00E+0 0.00E+0 0.00E+0 0.00E+0 0.00E+0 0.00E+0 0.00E+0 0.00E+0
RSF [MJ] 0.00E+0 0.00E+0 0.00E+0 0.00E+0 0.00E+0 0.00E+0 0.00E+0 0.00E+0 0.00E+0 0.00E+0 0.00E+0 0.00E+0
NRSF [MJ] 0.00E+0 0.00E+0 0.00E+0 0.00E+0 0.00E+0 0.00E+0 0.00E+0 0.00E+0 0.00E+0 0.00E+0 0.00E+0 0.00E+0
FW [m³] 2.57E-2 6.13E-4 5.20E-3 0.00E+0 0.00E+0 0.00E+0 0.00E+0 8.05E-5 5.29E-5 0.00E+0 6.12E-4 6.89E-5
PERE = Use of renewable primary energy excluding renewable primary energy resources used as raw materials; PERM = Use of
renewable primary energy resources used as raw materials; PERT = Total use of renewable primary energy resources; PENRE = Use of
non-renewable primary energy excluding non-renewable primary energy resources used as raw materials; PENRM = Use of non-
Caption
renewable primary energy resources used as raw materials; PENRT = Total use of non-renewable primary energy resources; SM = Use
of secondary material; RSF = Use of renewable secondary fuels; NRSF = Use of non-renewable secondary fuels; FW = Use of net fresh
water
RESULTS OF THE LCA – OUTPUT FLOWS AND WASTE CATEGORIES according to EN 15804+A1:
1 m² MASTERIMPACT®-RH (9 mm)
Parameter Unit A1-A3 A4 A5 B1 B2 B6 B7 C1 C2 C3 C4 D
HWD [kg] 2.87E-7 3.49E-7 1.72E-4 0.00E+0 0.00E+0 0.00E+0 0.00E+0 7.37E-11 3.01E-8 0.00E+0 4.56E-8 -1.00E-9
NHWD [kg] 4.66E-1 5.06E-4 3.75E-1 0.00E+0 0.00E+0 0.00E+0 0.00E+0 1.11E-4 4.36E-5 0.00E+0 1.18E+1 3.45E-3
RWD [kg] 3.76E-3 8.26E-6 4.50E-4 0.00E+0 0.00E+0 0.00E+0 0.00E+0 2.60E-5 7.13E-7 0.00E+0 5.20E-5 3.49E-5
CRU [kg] 0.00E+0 0.00E+0 0.00E+0 0.00E+0 0.00E+0 0.00E+0 0.00E+0 0.00E+0 0.00E+0 0.00E+0 0.00E+0 0.00E+0
MFR [kg] 0.00E+0 0.00E+0 2.03E-2 0.00E+0 0.00E+0 0.00E+0 0.00E+0 0.00E+0 0.00E+0 1.00E-1 0.00E+0 0.00E+0
MER [kg] 0.00E+0 0.00E+0 0.00E+0 0.00E+0 0.00E+0 0.00E+0 0.00E+0 0.00E+0 0.00E+0 0.00E+0 0.00E+0 0.00E+0
EEE [MJ] 0.00E+0 0.00E+0 0.00E+0 0.00E+0 0.00E+0 0.00E+0 0.00E+0 0.00E+0 0.00E+0 0.00E+0 0.00E+0 0.00E+0
EET [MJ] 0.00E+0 0.00E+0 0.00E+0 0.00E+0 0.00E+0 0.00E+0 0.00E+0 0.00E+0 0.00E+0 0.00E+0 0.00E+0 0.00E+0
HWD = Hazardous waste disposed; NHWD = Non-hazardous waste disposed; RWD = Radioactive waste disposed; CRU = Components
Caption for re-use; MFR = Materials for recycling; MER = Materials for energy recovery; EEE = Exported electrical energy; EEE = Exported
thermal energy
6. LCA: Interpretation
Looking at the overall lifecycle, for most of the impact For ADPe, the use of the stainless steel screws in A5
categories (except for ADPe, EP and ODP), the contributes most significantly to the results. The EP is
manufacturing (A1-A3) of MASTERIMPACT®-RH also strongly influenced by the landfilling of the
contributes to the largest share (> ~ 50 %) to the cellulose-containing materials. The powder mix finisher
environmental performance. contributes most significantly to the ODP of module
A5.
Interpretation of LCA-results in A1:
Within modules A1-A3, the pre-chains of the raw The LCA for MASTERIMPACT®-RH is mainly
material have the most important impact (contribution determined by the pre-chains of the following raw
> 50%) followed by the energy consumption for the materials: cement, cellulose and silica sand flour. The
production. Transport to site (A2) has a negligible contribution per impact category varies within these
influence on the overall LCA results (contribution < raw materials. Cement is most important for GWP,
2.5%). POCP and ADPe, whereas cellulose has a significant
impact on AP and EP. Compared to cement and
The re-emission of organic CO2 inherent in packaging cellulose, the contribution of silica sand is lower in all
materials (wooden pallets, cardboards) as well as in impact categories and only shows a relevant impact for
cellulose takes place in module A5, in which the ODP (contribution >25%).
packaging and the installation wastes are incinerated.
7. Requisite evidence
 At 5.6 μg/m³, the total VOC ("TVOC") after 3
7.1 Radioactivity days was below the limit of 10 mg/m³.
Radioactivity measurements confirm that no other
 At < 5 μg/m³, the total VOC ("TVOC") after 28
gamma emitters than those originating from the natural
days was below the limit of 1 mg/m³.
radiation sources are contained. The measured
radioactivity levels do not exceed the activity  At < 5 μg/m³, total SVOC after 28 days was
concentration indices as specified by the /Article 3 below the limit value of 0.1 mg/m³.
(Radiation Protection 112) for building products/  At > 5 μg/m³, the VOC individual substances
following the /Council Directive 96/29/. established after 28 days resulted in a rating
value R below the maximum limit of 1.
/Report on Radioactivity/
 At < 5 μg/m³, total individual VOC substances
7.2 Leaching without LCI value after 28 days were below
Leaching tests based on /EN 12457-2/ showed that no the limit value of 0.1 mg/m³
hazardous compounds were leached out.  At < 3 μg/m³, the formaldehyde concentration
after 28 days was below the limit of 120
/Report on Leaching/
μg/m³.
7.3 VOC emissions
/Report on VOC emissions/ The MASTERIMPACT®-RH product under review is
suitable for use in interior applications in accordance
Process: Testing the product emissions in accordance with /AgBB/ "Health-related Evaluation Procedure for
with the "Ausschuss zur gesundheitlichen Bewertung Volatile Organic Compounds Emissions (VOC and
von Bauprodukten" (/AgBB/) method SVOC) from Construction Products" in the version
dated May 2010.
Results:
 Carcinogens were not detected after 3 and 28
days.
8. References
Nachhaltiges Bauen (BNB)" Sustainable Building
Information Portal by the Federal Ministry of Transport,
Building and Urban Affairs (Bundesinstitut für Bau-,
/Article 3 (Radiation Protection 112) for building Stadt- und Raumforschung, BBSR)
products/ https://www.nachhaltigesbauen.de/baustoff-und-
Radiological Protection Principles concerning the gebaeudedaten/nutzungsdauern-von-bauteilen.html
Natural Radioactivity of Building Materials, published in
1999 by the Directorate-General Environment, Nuclear /Construction Products Regulation/
Safety and Civil Protection Regulation (EU) No 305/2011 of the European
Parliament and of the Council of 9 March 2011 laying
/AgBB/ down harmonised conditions for the marketing of
Ausschuss zur gesundheitlichen Bewertung von construction products and repealing Council Directive
Bauprodukten, AgBB (engl. German Committee 89/106/ EEC Text with EEA relevance
for Health-Related Evaluation of Building Products)
/Council Directive 96/29/
/BAM/ /Council Directive 96/29/Euratom/ of 13 May 1996
Material Testing Institute of the state of laying down basic safety standards for the protection of
Brandenburg/Berlin and the German Federal Institute the health of workers and the general public against
for Materials Research and Testing the dangers arising from ionizing radiation
/BBSR/ /DIN 4102-1/
BBSR table "Service lives of components for life cycle DIN 4102-1:1998, Fire behaviour of building materials
assessment according to Bewertungssystem
8 Environmental Product Declaration ETEX – MASTERIMPACT®-RH Fibre-Cement Drywall Panels
and elements - Classification of building materials -
Requirements and testing /ISO 9001/
UNI EN ISO 9001:2015 September 2015, Quality
/DIN 53436/ management systems - Requirements
DIN 53436-1:2015-12, Generation of thermal
decomposition products from materials for their
analytic-toxicological testing - Part 1: Decomposition /ISO 14001/
apparatus and determination of test temperature UNI EN ISO 14001:2015, Environmental management
systems - Requirements with guidance for use
/EN 12457-2/
NF EN 12457-2, December 2002, Characterization of /OHSAS 18001/
waste - Leaching - Compliance test for leaching of OHSAS 18001:2007, Occupational Health and Safety
granular waste materials and sludges - Part 2: one Management Certification
stage batch test at a liquid to solid ratio of 10 l/kg for
materials with particle size below 4 mm (without or with /Ordinance on Biocide Products/
size reduction) Regulation (EU) No 528/2012 of the European
Parliament and of the Council of 22 May 2012
/EN 12467/ concerning the making available on the market and
NF EN 12467, November 2012, Fibre-cement flat use of biocidal products
sheets - Product specification and test methods
/PCR Part A/
/EN 13501-1/ PCR Part A, Calculation rules for the LCA and
NF EN 13501-1+A1 February 2013, Fire classification requirements on the Background Report, Version 1.7,
of construction products and building elements - Part Institut Bauen und Umwelt e.V., www.ibu-epd.com,
1: classification using data from reaction to fire tests 2018
/EN 197-1/ /PCR Part B/
DIN EN 197-1:2011-11, Cement – Part 1: Composition, PCR Part B, Requirements on the EPD for Fibre
specifications and conformity criteria for common cement / Fibre concrete, Version 1.6, Institut Bauen
cement; German version EN 197-1:2011 und Umwelt e.V., www.bau-umwelt.com, 2017
/ETA 06/0207/ /REACH Regulation/
European Technical Assessment 06/0207 Version 01, Regulation (EU) No 1907/2006 of the
date of issue: 2018-06-25 European Parliament and of the Council of 18
December 2006 concerning the Registration,
/Eurofins Analyses pour l’Environnement/ Evaluation, Authorisation and Restriction of Chemicals
Eurofins Analyses pour l'Environnement France (REACH), establishing a European Chemicals Agency,
5, rue d'Otterswiller amending Directive 1999/45/EC and repealing Council
67700, Saverne Regulation (EEC) No 793/93 and Commission
France Regulation (EC) No 1488/94 as well as Council
Directive 76/769/EEC and Commission Directives
/Eurofins Product Testing A/S/ 91/155/EEC, 93/67/EEC, 93/105/EC and 2000/21/EC
Smedeskovvej 38
DK - 8464 /Report on Radioactivity/
Galten Date: 2 December 2011
Denmark Measuring agency: /SCK.CEN Laboratory for
Gammaspectrometry/, Mol, Belgium
/European Waste Index/ Protocol: Activity concentration index (ACI)[AR1]
European Waste Index provides an EU-wide common
terminology for waste classification. The index is in the /Report on Leaching/
Commission Decision of 3 May 2000 Date: 26 June 2015
Measuring agency: /Eurofins Analyses pour
/GaBi documentation/ l’Environnement/ France-Site de Saverne[AR2]
GaBi 8.7 data set documentation for the software
system and data bases, LBP, University of Stuttgart /Report on VOC emissions/
and thinkstep AG, Leinfelden-Echterdingen, 2018 Date: 29.11.2011
(http://www.gabi- Measuring agency: /Eurofins Product Testing A/S/
software.com/international/support/gabi/gabi-database- Smedeskovvej 38, 8464 Galten, Denmark;
2018-lci-documentation) Report no. G10208A
/GaBi ts software/ /SCK.CEN Laboratory for Gamma spectrometry/
GaBi Software-System and Database for Life SCK•CEN Research Center MolBoeretang 200
Cycle Engineering, 1992-2018, thinkstep AG, 2400 Mol
Leinfelden-Echterdingen, with acknowledgement of België
LBP University of Stuttgart, program version 8.7
9 Environmental Product Declaration ETEX – MASTERIMPACT®-RH Fibre-Cement Drywall Panels
Publisher
Institut Bauen und Umwelt e.V. Tel +49 (0)30 3087748- 0
Panoramastr. 1 Fax +49 (0)30 3087748- 29
10178 Berlin Mail info@ibu-epd.com
Germany Web www.ibu-epd.com
Programme holder
Institut Bauen und Umwelt e.V. Tel +49 (0)30 - 3087748- 0
Panoramastr 1 Fax +49 (0)30 – 3087748 - 29
10178 Berlin Mail info@ibu-epd.com
Germany Web www.ibu-epd.com
Author of the Life Cycle
Assessment Tel +49 711 341817-0
thinkstep AG Fax +49 711 341817-25
Hauptstraße 111- 113 Mail info@thinkstep.com
70771 Leinfelden-Echterdingen Web http://www.thinkstep.com
Germany
Owner of the Declaration
Etex Building Performance Tel +32 2 778 12 11
International Fax +32 2 778 12 12
Marcel Demonque 500 r Mail info@etexgroup.com
84915 Avignon Cedex 9 Web http://www.etexgroup.com
France
