ENVIRONMENTAL PRODUCT DECLARATION
as per ISO 14025 and EN 15804+A2
Owner of the Declaration ICDLI aisbl – International Committee of the Decorative Laminates
Industry
Programme holder Institut Bauen und Umwelt e.V. (IBU)
Publisher Institut Bauen und Umwelt e.V. (IBU)
Declaration number EPD-ICL-20220237-CBE1-EN
Issue date 18.11.2022
Valid to 17.11.2027
HPL-Compact
International Committee of the Decorative
Laminates Industry (ICDLI aisbl)
www.ibu-epd.com | https://epd-online.com
Umwelt Produktdeklaration Name des Herstellers – Name des Produkts
General Information
International Committee of the High Pressure Compact Laminate
Decorative Laminates Industry aisbl
(ICDLI)
Programme holder Owner of the declaration
IBU – Institut Bauen und Umwelt e.V. ICDLI aisbl – International Committee of the Decorative
Hegelplatz 1 Laminates Industry
10117 Berlin Rue de la presse 4
Germany 1000 Brussels/Belgium
Headoffice:
Mainzer Landstraße 55
60239 Frankfurt am Main/Germany
Declaration number Declared product / declared unit
EPD-ICL-20220237-CBE1-EN HPL-Compact according to EN 438-4 produced by
ICDLI aisbl members. The EPD applies to 1 m² of
Compact Laminate Panels without fire-retardant
properties with an average density of 1350 kg/m³.
This declaration is based on the product Scope:
category rules: The applicability of this document is restricted to HPL-
Laminates, 09.2022 Compact produced by member companies of the
(PCR checked and approved by the SVR) Laminate Association ICDLI aisbl.
Data has been provided by 10 member HPL-Compact
producing companies of the ICDLI aisbl for the year
Issue date
2021. These companies represent 75 % of the ICDLI
18.11.2022
aisbl members. The production volume of these
companies contributes more than 45 % to the HPL-
Valid to Compact production in Europe.
17.11.2027
The owner of the declaration shall be liable for the
underlying information and evidence; the IBU shall not
be liable with respect to manufacturer information, life
cycle assessment data and evidences.
The EPD was created according to the specifications
of EN 15804+A2. In the following, the standard will be
simplified as EN 15804.
Verification
The standard EN 15804 serves as the core PCR
Independent verification of the declaration and data
according to ISO 14025:2011
Dipl. Ing. Hans Peters internally x externally
(chairman of Institut Bauen und Umwelt e.V.)
Dr. Alexander Röder Dr. Stefan Diederichs
(Managing Director Institut Bauen und Umwelt e.V.)) (Independent verifier)
Product
Product description/Product definition mechanical fastening brackets to be used in invisible
This EPD describes HPL-Compact according to EN mounting systems.
438-4 (Compact HPL, thickness ≥ 2 mm) with a density
of at least 1350 kg/m³. Dimensions:
HPL-Compact is characterised by its aesthetic Length: up to 5600 mm
qualities, strength, durability and functional Width: up to 2200 mm
performance. HPL-Compact sheets are available in a
wide variety of colours, patterns and surface finishes. Thickness 2 ≤ t < 40 mm (HPL-Compact, EN 438-4)
They are resistant to wear, impact, scratching, A large number of HPL manufacturing plants are
moisture, heat, staining and light and possess good certified to ISO 9001 and/or ISO 14001.
hygienic and -antistatic properties. HPL-Compact is
easy to clean and maintain. For the placing on the market of HPL Compact Panels
HPL-Compact can be glued, riveted or screwed on in the European Union/European Free Trade
wooden or metallic substructures or anchored in Association (EU/EFTA) (with the exception of
2 Environmental Product Declaration ICDLI aisbl – HPL Compact Laminates
Switzerland) Regulation (EU) No. 305/2011 (CPR) Dimensional deviation: Length
+10/-0 mm
applies. HPL Compact Panels needs a Declaration of and width acc. to EN 438
Performance (DoP) taking into consideration EN 438-7 Formaldehyde emissions acc. to
< 100 μg/m3
:2005 and the CE-marking. For the application and use EN 717-1
the respective national provisions apply.
Application  Performance data of HPL Compact Panels in
HPL-Compact can be used for private and -residential accordance with the Declaration of
housing, hospitals and laboratories, public buildings, - Performance (DoP) with respect to its
railway stations, airport terminals/infrastructure, Essential Characteristics according to EN
transportation, -hotels, education, retail and 438-7:2005 apply.
commercial buildings, sport & recreation centres and  Voluntary data: EN 438-4:2016
industrial buildings.
The performance properties of HPL-Compact make
them suitable for use in a wide variety of interior
applications such as wall cladding, railing infill panels, Base materials/Ancillary materials
furniture, tables, desks, column cladding and lab More than 60 % of the HPL-Compact consists of
equipment, cubicles, ceilings, window sills, worktops, paper, and the remaining 30 to 40 % consists of cured
countertops, wash basins, etc. phenol resin for core layers and melamine resin for the
surface layer. HPL-Compact is produced in a high-
pressure process. Papers are impregnated with
Technical Data thermosetting resins and pressed together under
An extract of the technical properties of HPL-Compact simultaneous application of heat (temperature > 120
according to EN 438 part 4 is given in the following °C) and high specific pressure (≥ 5 MPa). This method
tables. For general purpose HPL-Compact used in produces a homogeneous, nonporous material with a
products without flame retardants, the following density ≥ 1350 kg/m³.
properties are given. HPL-Compact typically have two decorative sides.
For packaging the materials cardboard, wood/wooden
Constructional data pallets and polyethylene film are used.
Name Value Unit
Density ≥ 1350 kg/m³ This product HPL-Compact contains substances listed
Grammage 10.8 kg/m2 in the candidate list (date: 12.08.2022) exceeding 0.1
percentage by mass: No.
Resistance to surface wear (IP) revolution
≥ 150
acc. to EN 438 s
Reference service life
Resistance to scratches acc. to
≥ 2 rating Due to the wide range of applications, no single
EN 438
reference service life can be established. For
Resistance to impact (large mm drop
≥ 1800 information, the service life in standard applications
diameter ball) acc. to EN 438 height
can range from 20 to 50 years (ICDLI aisbl suggestion
Flexural strength acc. to EN 438 ≥ 80 N/mm²
based on expert judgment).
Modulus of elasticity acc. to EN
≥ 9000 N/mm2
438
Light resistance acc. to EN 438 ≥ 4 -
Dimensional deviation : Thickness
± 0.5 mm
tolerance acc. to EN 438
LCA: Calculation rules
Declared Unit
The declared unit is 1 m2 of HPL-Compact with 8 mm The EPD is representative for (of) the ICDLI
thickness and a density of at least 1350 kg/m³. The association. With regard to the variability compared to
declared unit refers to the HPL-Compact products the actual production, a slight variability can occur due
manufactured with phenolic-impregnated kraft paper to different production technologies and locations
core and melamine-impregnated decor paper. Special (different national energy mixes)
decors, fire retardants or alternative core production
technologies are not included. The declared unit refers
to the average HPL-Compact products manufactured System boundary
by ICDLI aisbl members (weighted average). Type of EPD: Cradle-to-gate with options.
Considered product stages:
Declared unit
Name Value Unit  Production of pre-products (e.g. resin
Declared unit 1 m2 ingredients and papers), extraction of energy
Grammage 10.8 kg/m2
carriers, raw material transportation,
manufacture of product and packaging
The EPD is an average product from factories of
materials are declared in modules A1-A3.
several HPL manufacturers. The averaging was done
by weighting according to the total production Modules A1-A3 also include the
quantities of the declared products of the member manufacturing and supply of energy.
companies.
3 Environmental Product Declaration ICDLI aisbl – HPL Compact Laminates
 The scenario for the transport of the product considering the biotic CO emissions
2
to the construction site is declared in module according to the incorporation on input side
A4.
 The treatment of packaging materials at The data collected by the manufacturers is based on
installation is declared in module A5. yearly production amounts. The production data refers
 The end-of-life scenarios include manual to the yearly consumption in 2021.
dismantling (C1), transportation to waste
Comparability
processing (C2), emissions and energy
Basically, a comparison or an evaluation of EPD data
requirements of combustion (C3). Credits for is only possible if all the data sets to be compared
electricity and thermal energy, which result were created according to EN 15804 and the building
from energy recovery in modules A5 and C3, context, respectively the product-specific
are declared in module D. characteristics of performance, are taken into account.
 The CO incorporation in the product (from
2 The GaBi ts software (CUP 2022.1) was used as
the sequestration in the paper material) is
background datasets.
considered. The C-balance is closed by
LCA: Scenarios and additional technical information
Characteristic product properties The transport to waste processing (module C2) is
Information on biogenic Carbon assumed to be 50 km.
Biogenic carbon is present in the product and the Name Value Unit
packaging materials. Collected separately 10.8 kg
Note: 1 kg biogenic Carbon is equivalent to 44/12 kg of Energy recovery 10.8 kg
CO
2
Reuse, recovery and/or recycling potentials (D),
Information on describing the biogenic Carbon Module D includes the potential benefits in form of
Content at factory gate energy recovery of the incineration process C3
Name Value Unit (incineration of HPL-Compact). A waste incineration
Biogenic Carbon Content in plant with R1-value > 0.6 is assumed.
2.94 kg C
product
Biogenic Carbon Content in
0.27 kg C
accompanying packaging
The following technical information is a basis for the
declared modules. This information can also be used
for developing specific scenarios in the context of a
building assessment for modules that are not declared
(MND)
Transport to the building site (A4)
Name Value Unit
Transport distance 100 km
Capacity utilisation (including
61 %
empty runs)
Gross density of products
1350 kg/m3
transported
Capacity utilisation volume factor 1 -
Installation into the building (A5)
Name Value Unit
Output substances following
waste treatment on site 0.73 kg
(packaging materials)
Packaging material:
polyethylene film : 0,08 kg/m²
cardboard: 0,05 kg/m²
wood (from pallets and fibreboard) : 0,60 kg/m²
End of life (C1-C4)
The deconstruction (module C1) is assumed to be
done manually (no environmental impact).
4 Environmental Product Declaration ICDLI aisbl – HPL Compact Laminates
LCA: Results
The following tables display the environmentally relevant results according to EN 15804 for 1 m² HPL-Compact.
DESCRIPTION OF THE SYSTEM BOUNDARY (X = INCLUDED IN LCA; ND = MODULE OR INDICATOR NOT
DECLARED; MNR = MODULE NOT RELEVANT)
BENEFITS AND
CONSTRUCTI LOADS
PRODUCT STAGE ON PROCESS USE STAGE END OF LIFE STAGE BEYOND THE
STAGE SYSTEM
BOUNDARIES
5 Environmental Product Declaration ICDLI aisbl – HPL Compact Laminates
lairetam
waR
ylppus tropsnarT
gnirutcafunaM
eht
morf
tropsnarT
etis
eht
ot
etag
ylbmessA esU
ecnanetniaM
riapeR
tnemecalpeR tnemhsibrufeR
ygrene
lanoitarepO esu
retaw
lanoitarepO esu
noitcurtsnoc-eD
noitilomed tropsnarT
gnissecorp
etsaW
lasopsiD -esueR -yrevoceR -gnilcyceR laitnetop
A1 A2 A3 A4 A5 B1 B2 B3 B4 B5 B6 B7 C1 C2 C3 C4 D
X X X X X ND ND MNR MNR MNR ND ND X X X X X
RESULTS OF THE LCA - ENVIRONMENTAL IMPACT according to EN 15804+A2: 1 m² HPL-Compact,
thickness 8.0 mm (10.8 kg/m²)
Core Indicator Unit A1-A3 A4 A5 C1 C2 C3 C4 D
GWP-total [kg CO2-Eq.] 5.44E+0 8.42E-2 1.19E+0 0.00E+0 4.21E-2 1.12E+1 0.00E+0 -5.28E+0
GWP-fossil [kg CO2-Eq.] 1.71E+1 8.06E-2 2.15E-1 0.00E+0 4.03E-2 3.64E-1 0.00E+0 -5.25E+0
GWP-biogenic [kg CO2-Eq.] -1.17E+1 3.67E-3 9.76E-1 0.00E+0 1.84E-3 1.08E+1 0.00E+0 -2.70E-2
GWP-luluc [kg CO2-Eq.] 1.34E-2 1.03E-6 4.12E-6 0.00E+0 5.16E-7 4.11E-5 0.00E+0 -5.80E-4
ODP [kg CFC11-Eq.] 1.09E-10 5.13E-15 1.04E-13 0.00E+0 2.56E-15 1.64E-12 0.00E+0 -3.57E-11
AP [mol H+-Eq.] 6.12E-2 2.43E-4 1.54E-4 0.00E+0 1.22E-4 9.31E-3 0.00E+0 -6.94E-3
EP-freshwater [kg P-Eq.] 1.60E-4 1.69E-8 2.54E-8 0.00E+0 8.43E-9 4.25E-7 0.00E+0 -7.27E-6
EP-marine [kg N-Eq.] 1.92E-2 1.14E-4 4.88E-5 0.00E+0 5.70E-5 4.41E-3 0.00E+0 -1.88E-3
EP-terrestrial [mol N-Eq.] 1.75E-1 1.25E-3 7.27E-4 0.00E+0 6.26E-4 5.11E-2 0.00E+0 -2.01E-2
POCP [kg NMVOC-Eq.] 5.13E-2 2.26E-4 1.34E-4 0.00E+0 1.13E-4 1.14E-2 0.00E+0 -5.26E-3
ADPE [kg Sb-Eq.] 2.65E-6 3.42E-9 2.54E-9 0.00E+0 1.71E-9 4.32E-8 0.00E+0 -7.96E-7
ADPF [MJ] 3.89E+2 1.13E+0 2.63E-1 0.00E+0 5.66E-1 5.31E+0 0.00E+0 -8.94E+1
[m³ world-Eq
WDP 2.17E+0 1.55E-4 1.13E-1 0.00E+0 7.77E-5 1.88E+0 0.00E+0 -5.63E-1
deprived]
GWP = Global warming potential; ODP = Depletion potential of the stratospheric ozone layer; AP = Acidification potential of land and water; EP =
Caption Eutrophication potential; POCP = Formation potential of tropospheric ozone photochemical oxidants; ADPE = Abiotic depletion potential for non-
fossil resources; ADPF = Abiotic depletion potential for fossil resources; WDP = Water (user) deprivation potential
RESULTS OF THE LCA - INDICATORS TO DESCRIBE RESOURCE USE according to EN 15804+A2: 1 m²
HPL-Compact, thickness 8.0 mm (10.8 kg/m²)
Indicator Unit A1-A3 A4 A5 C1 C2 C3 C4 D
PERE [MJ] 1.45E+2 4.27E-3 9.97E+0 0.00E+0 2.14E-3 1.17E+2 0.00E+0 -2.47E+1
PERM [MJ] 1.26E+2 0.00E+0 -9.91E+0 0.00E+0 0.00E+0 -1.16E+2 0.00E+0 0.00E+0
PERT [MJ] 2.71E+2 4.27E-3 6.00E-2 0.00E+0 2.14E-3 1.00E+0 0.00E+0 -2.47E+1
PENRE [MJ] 2.96E+2 1.13E+0 3.99E+0 0.00E+0 5.67E-1 9.55E+1 0.00E+0 -8.94E+1
PENRM [MJ] 9.39E+1 0.00E+0 -3.73E+0 0.00E+0 0.00E+0 -9.02E+1 0.00E+0 0.00E+0
PENRT [MJ] 3.89E+2 1.13E+0 2.63E-1 0.00E+0 5.67E-1 5.31E+0 0.00E+0 -8.94E+1
SM [kg] 2.76E+0 0.00E+0 0.00E+0 0.00E+0 0.00E+0 0.00E+0 0.00E+0 0.00E+0
RSF [MJ] 0.00E+0 0.00E+0 0.00E+0 0.00E+0 0.00E+0 0.00E+0 0.00E+0 0.00E+0
NRSF [MJ] 0.00E+0 0.00E+0 0.00E+0 0.00E+0 0.00E+0 0.00E+0 0.00E+0 0.00E+0
FW [m³] 8.93E-2 6.44E-6 2.67E-3 0.00E+0 3.22E-6 4.43E-2 0.00E+0 -2.37E-2
PERE = Use of renewable primary energy excluding renewable primary energy resources used as raw materials; PERM = Use of
renewable primary energy resources used as raw materials; PERT = Total use of renewable primary energy resources; PENRE = Use of
non-renewable primary energy excluding non-renewable primary energy resources used as raw materials; PENRM = Use of non-
Caption
renewable primary energy resources used as raw materials; PENRT = Total use of non-renewable primary energy resources; SM = Use
of secondary material; RSF = Use of renewable secondary fuels; NRSF = Use of non-renewable secondary fuels; FW = Use of net fresh
water
RESULTS OF THE LCA – WASTE CATEGORIES AND OUTPUT FLOWS according to EN 15804+A2:
1 m² HPL-Compact, thickness 8.0 mm (10.8 kg/m²)
Indicator Unit A1-A3 A4 A5 C1 C2 C3 C4 D
HWD [kg] 1.79E-6 3.74E-12 2.44E-11 0.00E+0 1.87E-12 6.63E-10 0.00E+0 -1.21E-8
NHWD [kg] 5.15E-1 1.06E-4 2.47E-2 0.00E+0 5.31E-5 1.36E-1 0.00E+0 -4.53E-2
RWD [kg] 5.54E-3 1.24E-6 1.42E-5 0.00E+0 6.21E-7 2.48E-4 0.00E+0 -7.08E-3
CRU [kg] 0.00E+0 0.00E+0 0.00E+0 0.00E+0 0.00E+0 0.00E+0 0.00E+0 0.00E+0
MFR [kg] 0.00E+0 0.00E+0 4.80E-2 0.00E+0 0.00E+0 0.00E+0 0.00E+0 0.00E+0
MER [kg] 0.00E+0 0.00E+0 0.00E+0 0.00E+0 0.00E+0 0.00E+0 0.00E+0 0.00E+0
EEE [MJ] 0.00E+0 0.00E+0 1.68E+0 0.00E+0 0.00E+0 2.21E+1 0.00E+0 0.00E+0
EET [MJ] 0.00E+0 0.00E+0 3.02E+0 0.00E+0 0.00E+0 3.92E+1 0.00E+0 0.00E+0
HWD = Hazardous waste disposed; NHWD = Non-hazardous waste disposed; RWD = Radioactive waste disposed; CRU = Components
Caption for re-use; MFR = Materials for recycling; MER = Materials for energy recovery; EEE = Exported electrical energy; EEE = Exported
thermal energy
RESULTS OF THE LCA – additional impact categories according to EN 15804+A2-optional:
1 m² HPL-Compact, thickness 8.0 mm (10.8 kg/m²)
Indicator Unit A1-A3 A4 A5 C1 C2 C3 C4 D
[Disease
PM 8.14E-7 1.29E-9 9.40E-10 0.00E+0 6.43E-10 2.77E-8 0.00E+0 -5.75E-8
Incidence]
[kBq U235-
IRP 9.58E-1 1.81E-4 2.25E-3 0.00E+0 9.04E-5 4.01E-2 0.00E+0 -1.20E+0
Eq.]
ETP-fw [CTUe] 1.38E+2 7.88E-1 1.37E-1 0.00E+0 3.94E-1 1.97E+0 0.00E+0 -1.97E+1
HTP-c [CTUh] 7.82E-9 1.46E-11 8.66E-12 0.00E+0 7.29E-12 1.29E-10 0.00E+0 -9.03E-10
HTP-nc [CTUh] 2.35E-7 7.13E-10 5.01E-10 0.00E+0 3.57E-10 4.77E-9 0.00E+0 -3.47E-8
SQP [-] 1.74E+3 3.12E-3 7.49E-2 0.00E+0 1.56E-3 1.25E+0 0.00E+0 -1.60E+1
PM = Potential incidence of disease due to PM emissions; IR = Potential Human exposure efficiency relative to U235; ETP-fw = Potential
Caption comparative Toxic Unit for ecosystems; HTP-c = Potential comparative Toxic Unit for humans (cancerogenic); HTP-nc = Potential
comparative Toxic Unit for humans (not cancerogenic); SQP = Potential soil quality index
Disclaimer 1 – for the indicator “Potential Human exposure efficiency relative to U235”.This impact category deals
mainly with the eventual impact of low dose ionizing radiation on human health of the nuclear fuel cycle. It does
not consider effects due to possible nuclear accidents, occupational exposure or radioactive waste disposal in
underground facilities. Potential ionizing radiation from the soil, radon and from some construction materials is
also not measured by this indicator.
Disclaimer 2 – for the indicators “abiotic depletion potential for non-fossil resources”, “abiotic depletion potential
for fossil resources”, “water (user) deprivation potential, deprivation-weighted water consumption”, “potential
comparative toxic unit for ecosystems”, “potential comparative toxic unit for humans – cancerogenic”, “Potential
comparative toxic unit for humans - not cancerogenic”, “potential soil quality index”. The results of this
environmental impact indicator shall be used with care as the uncertainties on these results are high as there is
limited experience with the indicator.
References
Standards DIN EN ISO 14001:2015-09, Environmental
management systems - Requirements with guidance
EN 438-2 for use
High-pressure decorative laminates (HPL) - Sheets
based on thermosetting resins (usually called ISO 14025
laminates) - Part 2: Determination of properties; EN EN ISO 14025:2011, Environmental labels and
438-2:2016+A1:2018 declarations — Type III environmental declarations —
Principles and procedures.
EN 438-3
High-pressure decorative laminates (HPL) - Sheets Further References
based on thermosetting resins (usually called
laminates) - Part 3: Classification and specifications for CPR
laminates less than 2 mm thick intended for bonding to Regulation (EU) No 305/2011 of the European
supporting substrates; EN 438-3: 2016 Parliament and of the Council of 9 March 2011 laying
down harmonised conditions for the marketing of
EN 438-7 construction products and repealing Council Directive
High-pressure decorative laminates (HPL) - Sheets 89/106/EEC
based on thermosetting resins (usually called
laminates) - Part 7: Compact laminate and HPL IBU 2021
composite panels for internal and external wall and Institut Bauen und Umwelt e.V.: General Instructions
ceiling finishes; EN 438-7:2005 for the EPD programme of Institut Bauen und Umwelt
e.V., Version 2.0, Berlin: Institut Bauen und Umwelt
EN 717-1 e.V., 2021
Wood-based panels - Determination of formaldehyde www.ibu-epd.com
release - Part 1: Formaldehyde emission by the
chamber method; EN 717-7:2004 GaBi
GaBi Software System and Database for Life Cycle
EN 15804 Engineering, 1992-2021, Sphera Solutions GmbH,
EN 15804:2012+A2:2019+AC:2021, Sustainability of Leinfelden-Echterdingen, with acknowledgement of
construction works — Environmental Product LBP University of Stuttgart, program version GaBi 10;
Declarations — Core rules for the product category of database version 2022.1
construction products.
GaBi documentation
ISO 9001 GaBi dataset documentation for the software system
DIN EN ISO 9001:2015-11, Quality management and databases, LBP, University of Stuttgart and
systems - Requirements Sphera Solutions GmbH, Leinfelden-Echterdingen,
2021.
ISO 14001 (http://www.gabi-software.com/support/gabi/gabi-
database-2021-lci-documentation/)
6 Environmental Product Declaration ICDLI aisbl – HPL Compact Laminates
PCR Part A
PCR - Part A: Calculation rules for the Life Cycle REACH
Assessment and Requirements on the Background Regulation (EC) No 1907/2006 concerning the
Report, version 1.6, Institut Bauen und Umwelt e.V., Registration, Evaluation, Authorisation and Restriction
www.bau-umwelt.com, 2017 of Chemicals (REACH)
PCR Part B
Part B: Requirements on the EPD for Laminates,
09/2022
7 Environmental Product Declaration ICDLI aisbl – HPL Compact Laminates
Publisher
Institut Bauen und Umwelt e.V. Tel +49 (0)30 3087748- 0
Hegelplatz 1 Fax +49 (0)30 3087748- 29
10117 Berlin Mail info@ibu-epd.com
Germany Web www.ibu-epd.com
Programme holder
Institut Bauen und Umwelt e.V. Tel +49 (0)30 - 3087748- 0
Hegelplatz 1 Fax +49 (0)30 – 3087748 - 29
10117 Berlin Mail info@ibu-epd.com
Germany Web www.ibu-epd.com
Author of the Life Cycle
Assessment Tel +49 711 341817-0
Sphera Solutions GmbH Fax +49 711 341817-25
Hauptstraße 111- 113 Mail info@sphera.com
70771 Leinfelden-Echterdingen Web www.sphera.com
Germany
Owner of the Declaration
ICDLI aisbl Headoffice Tel +49 69 2 71 05-31
Mainzer Landstraße 55 Fax N/A
60239 Frankfurt am Main Mail info@pro-kunststoff.de
Germany Web www.icdli.com
