ENVIRONMENTAL PRODUCT DECLARATION
as per ISO 14025 and EN 15804+A2
Owner of the Declaration voestalpine AG
Publisher Institut Bauen und Umwelt e.V. (IBU)
Programme holder Institut Bauen und Umwelt e.V. (IBU)
Declaration number EPD-VOE-20230456-IBA1-EN
Issue date 18/12/2023
Valid to 17/12/2028
Rail expansion joint - superstructure
voestalpine Turnout Technology Germany
GmbH
www.ibu-epd.com | https://epd-online.com
1. General Information
voestalpine Turnout Technology Germany Rail expansion joint - superstructure
GmbH
Programme holder Owner of the declaration
IBU – Institut Bauen und Umwelt e.V. voestalpine AG
Hegelplatz 1 voestalpine-Straße 3
10117 Berlin 4020 Linz
Germany Austria
Declaration number Declared product / declared unit
EPD-VOE-20230456-IBA1-EN 1 ton of rail expansion joint 60-600
This declaration is based on the product category rules: Scope:
Rails forming a track for vehicles, 01/08/2021 This EPD is based on a declared unit of 1 ton of rail expansion joint (REJ)
(PCR checked and approved by the SVR) of voestalpine Turnout Technology Germany GmbH produced at the
production sites in Butzbach and Brandenburg (Germany). The given
results refer to REJ 60-600 with an expansion length of 600 mm. In
Issue date addition conversion factors for REJ 60-300 and REJ 60-1200 with
respective expansion lenghts of 300 mm and 1200 mm are given in
18/12/2023
chapter 6. The EPD considers the superstructure of the rail expansion
joints without sleepers.
Valid to
The owner of the declaration shall be liable for the underlying information
17/12/2028 and evidence; the IBU shall not be liable with respect to manufacturer
information, life cycle assessment data and evidences.
The EPD was created according to the specifications of EN 15804+A2. In
the following, the standard will be simplified as EN 15804.
Verification
The standard EN 15804 serves as the core PCR
Independent verification of the declaration and data according to ISO
14025:2011
internally X externally
Dipl.-Ing. Hans Peters
(Chairman of Institut Bauen und Umwelt e.V.)
Florian Pronold Matthias Schulz,
(Managing Director Institut Bauen und Umwelt e.V.) (Independent verifier)
1 Environmental Product Declaration - voestalpine Turnout Technology Germany GmbH - Rail expansion joint - superstructure
2. Product
Constructional data
2.1 Product description/Product definition
The products of voestalpine Turnout Technology Germany Name Value Unit
GmbH are manufactured according to applicable European and Ballasted track or slab track type (e.g.,
Track form
international standards, guidelines and specifications. type Rheda 2000)
Usage of Eddy
is possible
For the use and application of the product, the respective brake
national provisions at the place of use apply, in Germany, for
1435 ± 1 (Accurate up to the pointed
example, the building codes of the federal states and the Track gauge mm
area of the switch rail)
corresponding national specifications.
Rail inclination 1:40, 1:20
Rail Expansion Joints (REJ, see EN 13232-8) are used in Curve Radius ≥ 2000 m
bridge constructions in order to compensate for the different Bridge
Steel or solid (concrete) structure
variations in length between the track system and the bridge, Construction
resulting from thermal forces, braking and acceleration forces ≤ 300 [REJ 60-300] (± 150 from neutral
as well as creeping and shrinkage of concrete. Expansion point) ≤ 600 [REJ 60-600] (± 300 from
mm
length neutral point) ≤ 1200 [REJ 60-1200] (±
REJ can be supplied for different expansion lengths. The basic 600 from neutral point)
geometry of the rail expansion joints is designed for 300 mm, Rail profile
600 mm and 1200 mm bridge expansion compensation. In (stock rail) 60E1 (UIC60)
special cases, the design and additional components can vary
Steel grade
due to customer specifications. R350HT (according to EN 13674-1)
(stock rail)
Rail profile
REJ can be manufactured and assembled according to the 60E1A1
(switch rail)
curvature and pre-bent at the factory (if required by design). A
possible preassembly takes place in a separate work step Steel grade
R350HT (according to EN 13674-2)
within the plants and is not taken into account in this EPD. (switch rail)
Turnout sleeper, length 3.00 m,
Sleeper type for
REJ system are usually installed on concrete sleepers and in connected with a steel strap at the
ballasted track
special cases on wooden sleepers or directly on special slab sleeper ends
track systems. 600 (Except the bridge gap or if
For representation, the data refers to a typical REJ 60-600 of Sleeper distance customer specification is required) mm
voestalpine Turnout Technology Germany GmbH. The sleepers
Rail fastening Vossloh Skl
or a slab track system are excluded from the scope.
Base plate
bold connection
2.2 Application fixation
The declared rail expansion joints of voestalpine Turnout Construction 16.880 [REJ 60-300] 17.200 [REJ 60-
mm
Technology Germany GmbH are mainly used in the following length of REJ 600] 17.550 [REJ 60-1200]
types of railway traffic: Bridge
temperature 70 (solid bridge), 90 (steel bridge) K
▪ High Speed Traffic difference ∆T
▪ Mixed Traffic
Performance data of the product with respect to its
▪ Urban Traffic
characteristics in accordance with the relevant technical
provision (no CE marking) depends on every individual product.
and there particularly in the following areas:
2.4 Delivery status
▪ bridge constructions
The products of voestalpine Turnout Technology Germany
▪ geologically unstable areas, where it´s required
GmbH are supplied in specified lengths. Rail expansion joints
2.3 Technical Data can be delivered as assembled onto different types of sleepers
or as half set of rail expansion devices assembled only on base
This EPD refers to the declared REJ 60-600 of voestalpine
plates for an assembly at trackside. Usually, the rail expansion
Turnout Technology Germany GmbH. The typical types of REJ
joints are delivered in a neutral position (adjusting value a = 0)
are presented in the following technical sheet.
or, on request, according to the position depending on the
temperature during installation at the construction site.
Customer supply can be just in time for every traffic station in
Europe.
2.5 Base materials/Ancillary materials
The REJ consist of different components. The main volume is
steel material like the rails and fixation parts. A small proportion
of the components at the fixation area are made of different
types of plastic materials (2.7 – 3.4 wt % of REJ).
This product contains substances listed in the candidate list
(05.08.2023) exceeding 0.1 percentage by mass: no.
2 Environmental Product Declaration - voestalpine Turnout Technology Germany GmbH - Rail expansion joint - superstructure
This product contains other carcinogenic, mutagenic, reprotoxic based on the applicable standards, guidelines and
(CMR) substances in categories 1A or 1B which are not on the specifications of the end customers.
candidate list, exceeding 0.1 percentage by mass: no.
2.11 Environment and health during use
Biocide products were added to this construction product or it No effects on human or animal health or harmful emissions into
has been treated with biocide products (this then concerns a the air, soil or water are to be expected during the use of the
treated product as defined by the (EU) Ordinance on Biocide rail expansion joints.
Products No. 528/2012): no.
2.12 Reference service life
2.6 Manufacture When used as intended, the lifespan of the declared products is
The steel and plastic parts are coming from external suppliers. based on the applicable standards and can be normally more
Rails are coming from the voestalpine Donawitz site. Further than 25 years. The service life of the product is optimized by
steel and plastic parts are coming from other external suppliers. regular maintenance performed by the end-user or
professionals in accordance with manufacturer installation and
Depending on customer specifications for REJ, the rails are maintenance manuals. Proper selection of the product can
then at voestalpine Turnout Technology Germany GmbH cut significantly increase the service life of REJ.
and prepared to achieve desired properties. This includes the
following works: With the preventive use of spare parts for individual
components, the life span of the whole system and main
▪ Precise shaping of the rails through vertical and horizontal components can increase.
straightening.
2.13 Extraordinary effects
▪ Cutting by sawing the rails on the required length.
▪ Drilling holes in the components for further processing. Fire
▪ Assembling the prefabricated individual parts. As the products do not contain any space for liquid or gas,
▪ Final acceptance of the system by the customer (on-site). environmental effects by losing these can be excluded.
▪ Storage and shipping of the REJ. Rail expansion joints are "non-flammable". No toxic gases and
vapours can arise.
The voestalpine Turnout Technology Germany GmbH Fire protection
production facilities are certified according to ISO 9001.
Name Value Unit
2.7 Environment and health during manufacturing Building material class n.a. -
The voestalpine Turnout Technology Germany GmbH Smoke gas development n.a. -
production facilities are certified according to ISO 14001, ISO Burning droplets n.a. -
50001 and occupational health- and safety assessment series
n.a. = not applicable
ISO 45001.
At the voestalpine Turnout Technology Germany GmbH sites,
Water
investments are made on a regular basis in an effort to expand
No negative effects on the environment are expected from
the environmental protection measures to reduce air and water
water (including flooding).
emissions to a minimum. Compliance with all statutory emission
limit values has been verified. All production systems approved
Mechanical destruction
in accordance with applicable environmental impact analyses
Unforeseeable mechanical effects on the declared product
are also inspected on a regular basis as part of environmental
would not have an environmental impact.
audits.
2.8 Product processing/Installation In case of mechanical overload (e.g. impact stress), the
products can be destroyed, but negative consequences for the
The processing and assembly of the declared products take
environment depend on the use of the defective products.
place in the factory or directly at the installation site of the REJ.
The installation is carried out in accordance with the applicable
2.14 Re-use phase
standards, guidelines and specifications of the customers.
Steel can either be reused or used as a valuable secondary
2.9 Packaging raw material in the steelmaking industry. Steel is a permanent
material that can be recycled as many times as necessary.
The products of voestalpine Turnout Technology Germany
GmbH are delivered mainly unpacked to the customer
Some components can be manufactured in a way, that steel
(fastened for transport with Signode or steel straps). In special
parts are vulcanised with elastomer plastic. There the recycling
cases are special packaging for sea freight required or other
has to be done according to national or local requirements.
methods the customer requires.
2.15 Disposal
When supplied without sleepers, respective transport
After the disassembly of REJ and the separation into the
protections shall be installed.
specific chemical materials (if it´s feasible), the steel parts and
Deliveries to the installation site or storage place can be made
plastic components can be recycled.
by rail, by truck or by plane.
The waste codes according to the European waste catalogue
Most materials used for transport can be reused for further
are:
deliveries.
2.10 Condition of use 07 02 13 waste plastic
17 04 05 iron and steel
When the rail expansion joints are in use, no changes in the
quality of the material are to be expected if they are used as
intended. The maintenance and inspection requirements are
3 Environmental Product Declaration - voestalpine Turnout Technology Germany GmbH - Rail expansion joint - superstructure
www.voestalpine.com/railwaysystems
2.16 Further information
More information on the product is available on the website
3. LCA: Calculation rules
3.1 Declared Unit Module D | Benefits and loads beyond the system
This environmental product declaration refers to a declared unit boundary
of 1 ton of 60-600 rail expansion joint. Module D declares the recycling of the recovered steel (95 % of
Declared unit the steel) and referring substitution potentials. In addition,
substitution potentials from energy recovery of the incineration
Name Value Unit
of the polymers are accounted for in this module. The energy
Declared unit 1 t
recovered from the incineration is assumed to substitute the
Weight per REJ (type 60-600) 8.91 t average European electricity grid mix and thermal energy from
Gross density 7850 kg/m³ natural gas.
Rail expansion joints are also produced with expansion lengths 3.3 Estimates and assumptions
of 300 mm and 1200 mm. Therefore chapter 6 presents
All assumptions are verified through detailed documentation
conversion factors for the environmental impacts of 1 ton REJ
and correspond to the best possible representation of reality
60-300 and REJ 60-1200. The respective total weight of the
based on the available data. Regional applicability of the used
REJ 60-300 and REJ 60-1200 arrives at 6.36 to and 9.32 to.
background data refers to average data under European or
German conditions taken from the GaBi database.
3.4 Cut-off criteria
3.2 System boundary
All inputs and outputs for which data are available are included
The life cycle assessment of rail expansion joints refers to a
in the LCA model. Data gaps are filled with conservative
cradle-to-gate analysis with modules (A1–A3 + C +D). The
assumptions from average data (when available) or with
following life cycle phases are part of the analysis:
generic data and are documented accordingly. Only data with a
contribution of less than 1 % were cut off. Ignoring such data is
Module A1–A3 | Production stage
justified based on the irrelevance of the expected effect.
The production stage includes the upstream burdens of raw
Processes, materials, or emissions known to make a significant
material supply (mainly steel), their transports and the
contribution to the environmental effects of the products under
manufacturing of the rail expansion joint at the production sites
examination have not been neglected. All relevant data were
of the voestalpine Turnout Technology Germany GmbH (TTG)
collected comprehensively. It is assumed that the data have
located at Butzbach and Brandenburg, Germany. The
been completely recorded and the overall total of ignored input
production sites are supplied with electricity from the regional
flows do not amount to more than 5 % of total energy and mass
power grid (residual grid mix) and thermal energy from natural
flows. Environmental impacts of machines, plant and
gas. The rails are delivered from upstream suppliers which are
infrastructure were not included
part of voestalpine group. Thus, the upstream environmental
impact of the production of the rails is represented based on 3.5 Background data
primary data. This study uses generic background data for the evaluation of
Rail expansion systems are delivered mainly unpacked to the upstream environmental impacts from GaBi-database 2022.2
customer. No packaging is considered in the LCA. and is modelled in GaBi-software version 10.
Module C1 | Deconstruction and demolition 3.6 Data quality
Energy demand for the deconstruction of the REJ from the The foreground data collected at voestalpine Turnout
track (e.g. loosening of screws) is strongly dependent on the Technology Germany GmbH are based on the quantities used
conditions at site and considered to be negligible. This results and volumes produced annually. All process data were
in a declaration of '0' in module C1. collected by voestalpine in the course of reporting to official
agencies. Data on material and energy use originate from
Module C2 | Transport to disposal material-specific throughput measurements of various
The transport to the disposal is accounted for assuming a processes as well as from controlling. The technological,
default scenario referring to a transport distance of 50 km via geographical and time related representativeness of the data
truck. base was kept in mind when selecting background data.
Whenever specific data were missing, either generic datasets
Module C3 | Waste processing or representative average data were used instead. The
The product flow that reaches Module D for recycling leaves the implemented GaBi background datasets are not more than ten
product system in C3. Crushing and sorting of the steel scrap years old.
are not included due to the insignificance of the expected
environmental impact. 3.7 Period under review
The plastic parts of the REJ are separated and processed in a Foreground data were collected in the 2021 production year,
waste incineration plant. Module C3 therefore accounts for the and the data are based on the volumes produced on an annual
environmental impacts from plastic waste incineration. basis.
3.8 Geographic Representativeness
Module C4 | Disposal
Module C4 refers to the emissions from the disposal of the Land or region, in which the declared product system is
losses from waste processing. The chosen scenario therefore manufactured, used or handled at the end of the product´s
includes the environmental burdens of landfilling of 5 % of the lifespan: Germany
steel.
4 Environmental Product Declaration - voestalpine Turnout Technology Germany GmbH - Rail expansion joint - superstructure
Therefore, the annual energy use is scaled down to the product
3.9 Allocation based on the processing time of the individual components.
The primary data for the upstream production of the steel billets This approach is considered as most representative for the
were allocated using the partitioning approach developed by allocation of the total energy input of the sites to the specific
worldsteel 2014 for calculating life cycle inventories of co- products. Land use was allocated to the product based on the
products in steel production, which is in line with the provisions mass of REJs produced.
of EN 15804. The so-called partitioning approach provides for
the allocation of environmental effects on the steelmaking 3.10 Comparability
process and the emerging byproducts based on physical Basically, a comparison or an evaluation of EPD data is only
relations. Material-inherent flow properties are, thus, taken into possible if all the data sets to be compared were created
account. Scrap used for the production is considered as according to EN 15804 and the building context, respectively
burdenfree input material. The net flows are calculated by the product-specific characteristics of performance, are taken
deducting the external steel scrap in A1–A3 from the overall into account.
mass of the product.
The GaBi background database was used to calculate the LCA
The specific evaluation of energy flows is not possible. (GaBi 10; 2022.2).
4. LCA: Scenarios and additional technical information
Reuse, recovery and/or recycling potentials (D), relevant
Characteristic product properties of biogenic carbon
scenario information
The declared products do not contain any biogenic carbon. No
packaging is considered in this study. Name Value Unit
Net flow of steel scrap 853 kg
The steel recycling scenario contains a recycling rate of 95 %.
Since voestalpine externally purchases scrap for steel
production, this is offset against the steel scrap for recycling
End of life (C1-C4) (net flow).
Name Value Unit
Collected separately waste type steel 972 kg
Recycling 95 % 924 kg
Landfilling 5 % 48 kg
Collected separately plastics 28 kg
Energy recovery 100 % 28 kg
5 Environmental Product Declaration - voestalpine Turnout Technology Germany GmbH - Rail expansion joint - superstructure
5. LCA: Results
The following table contains the LCA results for a declared unit of 1 ton of 60-600 rail expansion joint.
DESCRIPTION OF THE SYSTEM BOUNDARY (X = INCLUDED IN LCA; ND = MODULE OR INDICATOR NOT DECLARED; MNR =
MODULE NOT RELEVANT)
Benefits and
Construction loads beyond
Product stage Use stage End of life stage
process stage the system
boundaries
la ire ta m w a Ry lp p u s tro p s n a rT g n iru tc a fu n a M e h t m o rf tro p s n a rTe tis e h t o t e ta g y lb m e s s A e s U e c n a n e tn ia M ria p e R tn e m e c a lp e R tn e m h s ib ru fe R y g re n e la n o ita re p Oe s u re ta w la n o ita re p Oe s u n o itc u rts n o c -e Dn o itilo m e d tro p s n a rT g n is s e c o rp e ts a W la s o p s iD -e s u e R-y re v o c e R-g n ilc y c e Rla itn e to p
A1 A2 A3 A4 A5 B1 B2 B3 B4 B5 B6 B7 C1 C2 C3 C4 D
X X X MND MND MND MND MNR MNR MNR MND MND X X X X X
RESULTS OF THE LCA - ENVIRONMENTAL IMPACT according to EN 15804+A2: 1 ton rail expansion joint 60-600
Parameter Unit A1-A3 C1 C2 C3 C4 D
Global Warming Potential total (GWP-total) kg CO 2 eq 3.36E+03 0 3.03E+00 5.5E+01 2.33E+00 -1.5E+03
Global Warming Potential fossil fuels (GWP-fossil) kg CO 2 eq 3.36E+03 0 3.01E+00 5.5E+01 2.33E+00 -1.5E+03
Global Warming Potential biogenic (GWP-biogenic) kg CO 2 eq 5.41E+00 0 0 6.82E-03 0 6.29E-01
Global Warming Potential luluc (GWP-luluc) kg CO 2 eq 8.18E-01 0 2.02E-02 3.39E-04 1.41E-03 -3.32E-02
Depletion potential of the stratospheric ozone layer (ODP) kg CFC11 eq 1.82E-09 0 2.95E-13 6.66E-12 3.09E-12 -1.68E-10
Acidification potential of land and water (AP) mol H+ eq 8.23E+00 0 1E-02 9.47E-02 7.41E-03 -3.2E+00
Eutrophication potential aquatic freshwater (EP-freshwater) kg P eq 5.78E-03 0 1.07E-05 2.93E-06 1.8E-06 -3.02E-04
Eutrophication potential aquatic marine (EP-marine) kg N eq 1.99E+00 0 4.59E-03 4.85E-02 1.81E-03 -5.67E-01
Eutrophication potential terrestrial (EP-terrestrial) mol N eq 2.14E+01 0 5.14E-02 5.37E-01 1.98E-02 -4.99E+00
Formation potential of tropospheric ozone photochemical oxidants kg NMVOC
6.65E+00 0 9E-03 1.24E-01 5.71E-03 -2.29E+00
(POCP) eq
Abiotic depletion potential for non fossil resources (ADPE) kg Sb eq 1E-02 0 3.03E-07 2.09E-07 1.64E-07 -3.68E-03
Abiotic depletion potential for fossil resources (ADPF) MJ 3.61E+04 0 3.94E+01 2.84E+01 3.33E+01 -1.4E+04
m3 world eq
Water use (WDP) 1.82E+02 0 3.36E-02 6.13E+00 -2.22E-02 -2.77E+02
deprived
RESULTS OF THE LCA - INDICATORS TO DESCRIBE RESOURCE USE according to EN 15804+A2: 1 ton rail expansion joint
60-600
Parameter Unit A1-A3 C1 C2 C3 C4 D
Renewable primary energy as energy carrier (PERE) MJ 1.95E+03 0 2.73E+00 3.83E+00 2.72E+00 7.41E+02
Renewable primary energy resources as material utilization
MJ 0 0 0 0 0 0
(PERM)
Total use of renewable primary energy resources (PERT) MJ 1.95E+03 0 2.73E+00 3.83E+00 2.72E+00 7.41E+02
Non renewable primary energy as energy carrier (PENRE) MJ 3.55E+04 0 3.96E+01 7.69E+02 3.33E+01 -1.4E+04
Non renewable primary energy as material utilization (PENRM) MJ 7.41E+02 0 0 -7.41E+02 0 0
Total use of non renewable primary energy resources (PENRT) MJ 3.62E+04 0 3.96E+01 2.84E+01 3.33E+01 -1.4E+04
Use of secondary material (SM) kg 2.24E+02 0 0 0 0 8.53E+02
Use of renewable secondary fuels (RSF) MJ 0 0 0 0 0 0
Use of non renewable secondary fuels (NRSF) MJ 0 0 0 0 0 0
Use of net fresh water (FW) m3 8.08E+00 0 3.15E-03 1.45E-01 4.67E-04 -6.31E+00
RESULTS OF THE LCA – WASTE CATEGORIES AND OUTPUT FLOWS according to EN 15804+A2:
1 ton rail expansion joint 60-600
Parameter Unit A1-A3 C1 C2 C3 C4 D
Hazardous waste disposed (HWD) kg 3.58E-06 0 2.09E-10 4.67E-09 5.03E-09 -1.61E-07
Non hazardous waste disposed (NHWD) kg 9.1E+01 0 6.45E-03 2.22E+00 4.87E+01 2.05E+02
Radioactive waste disposed (RWD) kg 5.22E-01 0 7.34E-05 7.65E-04 4.01E-04 -3.1E-02
Components for re-use (CRU) kg 0 0 0 0 0 0
Materials for recycling (MFR) kg 1.53E+02 0 0 9.24E+02 0 0
Materials for energy recovery (MER) kg 0 0 0 0 0 0
Exported electrical energy (EEE) MJ 0 0 0 1.1E+02 0 0
Exported thermal energy (EET) MJ 0 0 0 1.97E+02 0 0
RESULTS OF THE LCA – additional impact categories according to EN 15804+A2-optional:
1 ton rail expansion joint 60-600
Parameter Unit A1-A3 C1 C2 C3 C4 D
Disease
Incidence of disease due to PM emissions (PM) ND ND ND ND ND ND
incidence
6 Environmental Product Declaration - voestalpine Turnout Technology Germany GmbH - Rail expansion joint - superstructure
Human exposure efficiency relative to U235 (IR) kBq U235 eq ND ND ND ND ND ND
Comparative toxic unit for ecosystems (ETP-fw) CTUe ND ND ND ND ND ND
Comparative toxic unit for humans (carcinogenic) (HTP-c) CTUh ND ND ND ND ND ND
Comparative toxic unit for humans (noncarcinogenic) (HTP-nc) CTUh ND ND ND ND ND ND
Soil quality index (SQP) SQP ND ND ND ND ND ND
The additional and optional impact categories according to EN 15804+A2 are not declared, as the uncertainty of these indicators is to
be classified as high.
Disclaimer – for the indicators 'abiotic depletion potential for non-fossil resources', 'abiotic depletion potential for fossil resources',
'water (user) deprivation potential, deprivation-weighted water consumption', 'potential comparative toxic unit for ecosystems', 'potential
comparative toxic unit for humans – cancerogenic', 'Potential comparative toxic unit for humans - not cancerogenic', 'potential soil
quality index'.
The results of this environmental impact indicator shall be used with care as the uncertainties on these results are high as there is
limited experience with the indicator.
6. LCA: Interpretation
The following interpretation contains a summary of the LCA expansion joint.
results referenced to a declared unit of 1 ton of 60-600 rail
The comparison of the products' life cycle phases shows a In addition, the upstream supply chain of the rails also plays an
clear dominance of the production phase (modules A1–A3). important role in most indicators, especially in the case of
eutrophication potential freshwater (EP-freshwater). The main
Environmental impacts in module C3 mainly refer to emissions influence of the rails on the EP-freshwater stems from the
from the energetic treatment of the polymers in a waste upstream supply chain of the steel billets used for
incineration plant. Module C4 declares impacts from landfilling manufacturing of the rails.
of steel losses making up a minor fraction of the total
environmental impact of the panels. A comparison of the different REJ types shows a deviation of
less than 2 % for most environmental impact indicators when
As a result of material recyclability, the steel fraction removed at scaled to 1 ton of REJ. For the indicators majorly influenced by
the end of life can substitute primary steel. Module D shows the upstream supply chain of the rails, the variance of the
the recycling potential of steel at the end of its product life. This results is comparably higher for the REJ 60-300, since the
results in potentials ("benefits") from the substitution of primary weight share of the rails is higher for this REJ type.
steel. In addition, the incineration of the polymers in the product
results in substitution potentials from energy recovery. In the following table conversion factors for the environmental
impacts of REJ 60-300 and REJ 60-1200 are shown:
The hot-spot analysis of the production phase shows the
production of the support point as a main contributor to all
impact categories except for eutrophication potential freshwater
(EP-freshwater). The high influences from the support point
result from the upstream supply chain of steel, constituting the
main material for the support point. The comparably high
contribution to the potential abiotic depletion of minerals and
metals (ADPE) can be traced back to the additional use of zinc
for the galvanization for some of the steel components.
7 Environmental Product Declaration - voestalpine Turnout Technology Germany GmbH - Rail expansion joint - superstructure
To obtain the specific results per to for the respective REJ, the
respective conversion factor must be multiplied with the results
in module A1–A3 from chapter 5 of this EPD.
7. Requisite evidence
Not relevant for this EPD.
8. References
Standards Further references
EN 13232-8 Candidate List
EN 13232-8:2012-01, Railway applications – Track – Switches Candidate List of Substances of Very High Concern (ECHA
and Crossings – Part 8: Expansion devices. Candidate List) of 05.08.2023, published in accordance with
Article 59 (10) of the REACH Regulation Helsinki: European
EN 13674-1 Chemicals Agency.
EN 13674-1:2011+A1:2017, Railway applications – Track – Rail
– Part 1: Vignole railway rails 46 kg/m and above. European Waste Catalogue
European Waste Catalogue (EWC) Ordinance of December
EN 13674-2 10th, 2001 (Federal Law Gazette I p. 3379), last amended by
EN 13674-2:2020-01, Railway applications - Track - Rail - Part Article 1 of the Ordinance of June 30th, 2020 (Federal Law
2: Switch and crossing rails used in conjunction with Vignole Gazette I p. 1533).
railway rails 46 kg/m and above.
GaBi
EN 15804 GaBi 10, Software-System and Database for Life Cycle
DIN EN 15804:2012+A2:2019+AC:2021, Sustainability of Engineering. DB 2022.2. Sphera, 1992-2022. Available at:
construction works - Environmental product declarations - Core https://sphera.com/life-cycle-assessment-lca-software/
rules for the product category of construction products.
IBU 2021
ISO 9001 Institut Bauen und Umwelt e.V.: General Instructions for the
DIN EN ISO 9001:2015, Quality management systems – EPD programme of Institut Bauen und Umwelt e.V., Version
Requirements. 2.0, Berlin: Institut Bauen und Umwelt e.V., 2021 www.ibu-
epd.com.
ISO 14001
DIN EN ISO 14001:2015, Environmental management systems ökobaudat 2022
– Requirements with guidance for use. ökobaudat 2022, EN 15804 and BNB compliant data for more
than 700 building products. Federal Ministry of the Interior,
ISO 14025 Building and Community.
DIN EN ISO 14025:2011, Environmental labels and
declarations – Type III environmental declarations – Principles Ordinance on Biocide Products
and procedures. Regulation (EU) No 528/2012 of the European Parliament and
of the Council of 22 May 2012 concerning the making available
ISO 14044 on the market and use of biocidal products.
ISO 14044:2006, Environmental Management – Life cycle
assessment – Requirements and guidelines. PCR Part A
Product category rules for building-related products and
ISO 45001 services. Part A: Calculation rules for the life cycle assessment
ISO 45001:2018, Occupational Health and Safety Management and requirements on the project report according to
Systems – Requirements with guidance for use. EN15804+A2:2019. Version 1.3, Berlin: Institut Bauen und
Umwelt e.V. (Hrsg.), 2022.
ISO 50001
ISO 50001:2018, Energy management systems – PCR: Rails forming a track for vehicles
Requirements with guidance for use. Institut Bauen und Umwelt e.V. (IBU), 2023. Product Category
8 Environmental Product Declaration - voestalpine Turnout Technology Germany GmbH - Rail expansion joint - superstructure
Rules for Building-Related Products and Services. Part B: worldsteel 2014
Requirements on the EPD for Rails forming a track for vehicles. World Steel Association, February 14, 2014: A methodology to
Version v4, 05.07.2023. determine the LCI of steel industry co-products.
9 Environmental Product Declaration - voestalpine Turnout Technology Germany GmbH - Rail expansion joint - superstructure
Publisher
Institut Bauen und Umwelt e.V. +49 (0)30 3087748- 0
Hegelplatz 1 info@ibu-epd.com
10117 Berlin www.ibu-epd.com
Germany
Programme holder
Institut Bauen und Umwelt e.V. +49 (0)30 3087748- 0
Hegelplatz 1 info@ibu-epd.com
10117 Berlin www.ibu-epd.com
Germany
Author of the Life Cycle Assessment
Daxner & Merl GmbH +43 676 849477826
Schleifmühlgasse 13/24 office@daxner-merl.com
1040 Wien www.daxner-merl.com
Austria
Owner of the Declaration
voestalpine AG +43/50304/15-0
voestalpine-Straße 3 info@voestalpine.com
4020 Linz www.voestalpine.com
Austria
10 Environmental Product Declaration - voestalpine Turnout Technology Germany GmbH - Rail expansion joint - superstructure
