ENVIRONMENTAL PRODUCT DECLARATION
as per ISO 14025 and EN 15804+A2
Owner of the Declaration JANSEN AG
Publisher Institut Bauen und Umwelt e.V. (IBU)
Programme holder Institut Bauen und Umwelt e.V. (IBU)
Declaration number EPD-JAN-20230115-CBA1-EN
Issue date 20.10.2023
Valid to 19.10.2028
Janisol Arte 66 window width x height: 1230mm x 1480mm
Jansen AG
www.ibu-epd.com | https://epd-online.com
General Information
Jansen AG Janisol Arte 66 window width x height: 1230mm x
1480mm
Programme holder Owner of the declaration
IBU – Institut Bauen und Umwelt e.V. JANSEN AG
Hegelplatz 1 Industriestrasse 34
10117 Berlin 9463 Oberriet
Germany Switzerland
Declaration number Declared product / declared unit
EPD-JAN-20230115-CBA1-EN 1 m2 Janisol Arte 66 window with a grammage of 47.69 kg/m². The actual
reference size of the declared window has dimensions of width x height:
1230 mm x 1480 mm.
This declaration is based on the product category rules: Scope:
Windows and doors , 01.08.2021 The environmental product declaration refers to a window type Janisol Arte
(PCR checked and approved by the SVR) 66 in specific dimension width x height. The characteristic values used for
the system components Janisol Arte 66 in the LCA are provided by Jansen
AG.
Issue date
The declared product is defined according to the profile series and product
20.10.2023
characteristics.
The location of the production site is Oberriet/ Switzerland.
Valid to
This EPD was created with the help of a semi-automatic LCA-Tool.
19.10.2028 The owner of the declaration shall be liable for the underlying information
and evidence; the IBU shall not be liable with respect to manufacturer
information, life cycle assessment data and evidences.
The EPD was created according to the specifications of EN 15804+A2. In
the following, the standard will be simplified as EN 15804.
Verification
The standard EN 15804 serves as the core PCR
Independent verification of the declaration and data according to ISO
14025:2011
Dipl.-Ing. Hans Peters internally X externally
(Chairman of Institut Bauen und Umwelt e.V.)
Florian Pronold Matthias Klingler,
(Managing Director Institut Bauen und Umwelt e.V.) (Independent verifier)
1 Environmental Product Declaration - Jansen AG - Janisol Arte 66 window width x height: 1230mm x 1480mm
Product
According to the CE marking, the following structural data for
Product description/Product definition the element must be stated:
With Janisol Arte 66, the basic depth of 66 mm enables the use
Constructional data
of higher glazing thickness with a sash height of up to 2300
mm. It is possible to have a tilt-and-turn opening type, even with Name Value Unit
the special requirements of listed buildings for narrow frames. Resistance to wind load acc. to EN
C5 class
Fabrication with push-in gasket or dry glazing takes place in the 12210
usual way, as with our other steel profile systems – this ensures Water tightness acc. to EN 12208 9A class
a high level of process reliability. This declaration describes the
Sound insulation class acc. to EN up to Rw 47 dB
following element in Janisol Arte: -
EN ISO 10140 (-2; -7)
Product: Janisol Arte 66
Heat transfer coefficient acc. to DIN
Width x height: 1230mm x 1480mm 1.6 W/(m2K)
EN ISO 10077-2
Face width sash: 68mm / transom 40mm
Basic depth: 66mm / sash depth: 70mm Air permeability acc. to EN 12207 4 class
CE marking according to EN 14351-1 Mechanical strength acc. to EN
4 class
13115
The products require a declaration of performance taking into Impact resistance acc. to EN 13049 4 class
account the harmonized product standard EN 14351-1 windows
Product according to the CPR, based on EN: Performance data
and doors and a CE marking. The respective national
of the product in accordance with the declaration of
regulations apply to the use. With this declaration the following
performance with respect to its essential characteristics
element is declared:
according to EN 14351-1, windows. Other constructional data
are not relevant for this product.
Base materials/Ancillary materials
JANSEN Janisol Arte 66 window is made of the following
materials:
• Glazing approx. 53%
• Steel approx. 30%
• Plastics and fillers approx. 13%
• Fittings approx. 4%
• Stainless steel < 1%
• Aluminium < 1%
The percentages relate to the most frequently sold product with
an opening of 1.82 m2. The percentages stated may vary
depending on the product type and dimensions.
Does the product or at least one part product contain materials
from the ECHA candidate list of materials which are especially
problematic for approval: Substances of Very High Concern –
SVHC (date 17.01.2023) above a mass % of 0.1: no.
This product/article/at least one partial article contains other
CMR substances in categories 1A or 1B which are not on the
candidate list, exceeding 0.1 percentage by mass: no.
Biocide products were added to this construction product or it
has been treated with biocide products (this then concerns a
treated product as defined by the (EU) Ordinance on Biocide
Products No. 528/2012): no.
Reference service life
According to SBR 2011 regarding the specific material
Application characteristics of steel windows and doors, the reference
The Janisol Arte 66 opening element can be integrated for service life is 75 years (SBR 2011). The practical service life
building ventilation and light transmission. may well be longer. Conditions for a long service life are regular
maintenance, care and upkeep of the product. The specified
Technical Data
service life is independent of the manufacturer's warranty.
LCA: Calculation rules
Declared unit
Declared Unit
The declared unit is a 1 m2 of Janisol Arte 66 window element.
The actual reference size of the declared window element has
dimensions of 1230 mm x 1480 mm.
2 Environmental Product Declaration - Jansen AG - Janisol Arte 66 window width x height: 1230mm x 1480mm
Name Value Unit Scenario 1: 100% thermal treatment of all raw materials with
Grammage 47.69 kg/m2 heating value including plastic system parts and 100%
recycling of metal system components (C3/1). Landfill of all
Declared unit 1 m2
materials without heating value (except metals) including
Layer thickness 0.066 m glazing (C4/1).
Scenario 2 (module C3/2): 100% recycling of plastic system
For inhomogeneous components made of different materials,
parts and 100% recycling of metal system components. Landfill
the conversion to other dimensions with factors leads to
of all materials without heating value (except metals) including
deviations compared to the exact calculation. The frame
glazing (C4/2).
percentage is 18.55% and the ground reference is 0.08118m².
Modules C4/1 & C4/2 are identical.
System boundary
Type of EPD according to EN 15804: "cradle to gate with EoL scenario 1 (modules C3/1 and C4/1)
options, modules C1–C4, and module D". The following Collected separately waste type (window element) 47.69 kg
modules are declared: A1–A3, C, D and additional modules: A4 Recycling (C3/1) 15.92 kg
+ A5. Energy recovery (C3/1) 3.26 kg
Landfilling (C4/1) 28.7 kg
Production (modules A1-A3):
EoL scenario 2 (modules C3/2 and C4/2)
This module considers the provision of all relevant window Collected separately (window element) 47.69 kg
components (i.e. metal profiles/ components, glass units and Recycling (C3/2) 18.99 kg
plastic parts/profiles) and raw materials including their transport Energy recovery (C3/2) 0.19 kg
to the declared production plant. This considers the Landfilling (C4/2) 28.70 kg
manufacturing and assembly of these components, including
waste processing up to the end-of-waste state. The impact of
packaging materials is also covered by this module. Benefits and loads beyond the product system boundary
(module D):
Transport to the construction site (module A4):
Considers credits and loads from the recycling of the metal
A distance of 100 km is considered for the transport of the components (duplicated in D/1 and D/2) and the recycling of
packed finished product via truck. The transport distance can the plastic system parts/profiles (D/2). Avoided burdens from
be modified project-specific if required by linear scaling. the thermal treatment of all raw materials with heating value
(including plastic system parts/ profiles) (D/1) and packaging
Installation (module A5): treatment (duplicated in D/1 and D/2) under European
conditions are considered. This affects only the rate of primary
Treatment and disposal of packaging material is considered in materials (no secondary materials).
this module. Credits for potential avoided burdens due to
Geographic Representativeness
energy substitution of electricity and thermal energy generation
Land or region, in which the declared product system is
are declared in module D under European conditions and
manufactured, used or handled at the end of the product´s
affects only the rate of primary materials (no secondary
lifespan: Europe
materials).
EoL stage (modules C1-C4):
Comparability
Basically, a comparison or an evaluation of EPD data is only
Module C1 - considers manual deconstruction (without
possible if all the data sets to be compared were created
environmental burdens).
according to EN 15804 and the building context, respectively
Module C2 - considers 50 km truck transport to waste
the product-specific characteristics of performance, are taken
processing. The transport distance can be modified project-
into account. The following background database has been
specific if required by linear scaling.
used for the LCA calculation: Sphera LCA software (GaBi ts)
Modules C3 and C4 - consider waste processing and/or
content update package (CUP) version 2022.2
disposal with the following scenarios:
LCA: Scenarios and additional technical information
Characteristic product properties of biogenic carbon The following technical information is a basis for the declared
No biogenic carbon is reported in the product. The biogenic modules. The values refer to the declared unit of 1 m2 of
carbon content in the accompanying packaging for 1 m2 Janisol Janisol Arte 66 window.
Arte 66 window is declared below.
Transport to the building site (A4)
Information on describing the biogenic Carbon Content at
Name Value Unit
factory gate
Litres of fuel 0.0939 l/100km
Name Value Unit
Transport distance 100 km
kg
Biogenic carbon content in product - Capacity utilisation (including empty runs) 61 %
C
Gross weight of packed products transported 47.71 kg
Biogenic carbon content in accompanying kg
0.00804
packaging C
Installation into the building (A5)
Note: 1kg of biogenic carbon is equivalent to 44/12 kg of CO2.
3 Environmental Product Declaration - Jansen AG - Janisol Arte 66 window width x height: 1230mm x 1480mm
Name Value Unit EPD is currently considered a scenario that is not widely
available in reality due to economic viability limitations
Polyethylene (waste packaging to incineration) 0.00173 kg
associated with higher costs of sorting smaller shares of
Cardboard box (waste packaging to incineration) 0.00829 kg
plastics such as those present in the declared product.
Wood (waste packaging to incineration) 0.0109 kg
Name ValueUnit
According to SBR 2011 regarding the specific material
EoL scenario 1 (modules C3/1 and C4/1)
characteristics of steel windows and doors, the reference
Collected separately waste type (window element) 47.69 kg
service life is 75 years (SBR 2011). The practical service life
Recycling (C3/1) 15.92 kg
may well be longer. Conditions for a long service life are regular
maintenance, care and upkeep of the product. The specified Energy recovery (C3/1) 3.26 kg
service life is independent of the manufacturer's warranty. Landfilling (C4/1) 28.7 kg
EoL scenario 2 (modules C3/2 and C4/2)
Collected separately (window element) 47.69 kg
Reference service life Recycling (C3/2) 18.99 kg
Energy recovery (C3/2) 0.19 kg
Name Value Unit Landfilling (C4/2) 28.70 kg
Life Span (according to SBR 2011) 75 a
Reuse, recovery and/or recycling potentials (D), relevant
Reference service life according to SBR 2011. scenario information
End of life (C1-C4) Module D includes the credits and loads from the recycling of
the metal components (duplicated in D/1 and D/2) and the
For the End-of-Life stage two scenarios are considered.
recycling of the plastic system parts/profiles (D/2). Avoided
Scenario 1 considers 100% thermal treatment of all raw
burdens from the thermal treatment of all raw materials with
materials with heating value including plastic system parts and
heating value (including plastic system parts/profiles) (D/1) and
100% recycling of metal system components (C3/1). Landfill of
packaging treatment (duplicated in D/1 and D/2) under
all materials without heating value (except metals) including
European conditions are considered. This affects only the rate
glazing (C4/1). Scenario 2 considers 100% recycling of plastic
of primary materials (no secondary materials). A waste
system parts and 100% recycling of metal system components
incineration plant with R1-value > 0.6 is assumed.
(C3/2). Landfill of all materials without heating value (except
metals) including glazing (C4/2). Modules C4/1 and C4/2 are
For recycling, a collection rate of 100% is considered.
identical. The recycling of plastics scenario declared in this
4 Environmental Product Declaration - Jansen AG - Janisol Arte 66 window width x height: 1230mm x 1480mm
LCA: Results
Results provided in this section are presented in relation to 1 m2 of window type Jansen Janisol Arte 66 (reference dimensions 1230
mm x 1480 mm).
For the End-of-Life stage, two scenarios are considered:
C3/1 - considers 100% recycling of metal system components (duplicated in D/1 and D/2) and 100% thermal treatment of all raw
materials with heating value including plastic system parts.
C3/2 - considers 100% recycling of metal system components (duplicated in D/1 and D/2) and 100% recycling of plastic system parts.
C4/1 and C4/2 - considers landfill of all materials without heating value (except metals) including glazing. Modules C4/1 and C4/2 are
identical.
D/1 - considers credits and loads from the recycling of the metal components (duplicated in D/1 and D/2). Avoided burdens from
packaging treatment (duplicated in D/1 and D/2) and thermal treatment of all raw materials with heating value (including plastic system
parts/profiles) are considered.
D/2 - considers credits and loads from the recycling of the metal components (duplicated in D/1 and D/2) and the recycling of the
plastic system parts/profiles. Avoided burdens from packaging treatment (duplicated in D/1 and D/2) are considered.
DESCRIPTION OF THE SYSTEM BOUNDARY (X = INCLUDED IN LCA; ND = MODULE OR INDICATOR NOT DECLARED; MNR =
MODULE NOT RELEVANT)
Benefits and
Construction loads beyond
Product stage Use stage End of life stage
process stage the system
boundaries
la ire ta m w a Ry lp p u s tro p s n a rT g n iru tc a fu n a M e h t m o rf tro p s n a rTe tis e h t o t e ta g y lb m e s s A e s U e c n a n e tn ia M ria p e R tn e m e c a lp e R tn e m h s ib ru fe R y g re n e la n o ita re p Oe s u re ta w la n o ita re p Oe s u n o itc u rts n o c -e Dn o itilo m e d tro p s n a rT g n is s e c o rp e ts a W la s o p s iD -e s u e R-y re v o c e R-g n ilc y c e Rla itn e to p
A1 A2 A3 A4 A5 B1 B2 B3 B4 B5 B6 B7 C1 C2 C3 C4 D
X X X X X MND MND MNR MNR MNR MND MND X X X X X
RESULTS OF THE LCA - ENVIRONMENTAL IMPACT according to EN 15804+A2: 1 m2 Janisol Arte 66 window (47.69 kg/m2)
Parameter Unit A1-A3 A4 A5 C1 C2 C3/1 C3/2 C4/1 C4/2 D/1 D/2
GWP-total kg CO 2 eq 8.77E+01 2.88E-01 3.52E-02 0 1.44E-01 7.44E+00 1.44E-01 4.3E-01 4.3E-01 -1.45E+01 -1.53E+01
GWP-fossil kg CO 2 eq 8.73E+01 2.85E-01 5.99E-03 0 1.43E-01 7.44E+00 1.44E-01 4.28E-01 4.28E-01 -1.45E+01 -1.53E+01
GWP-
biogenic kg CO 2 eq 3.59E-01 1.2E-03 2.92E-02 0 6.02E-04 4.72E-04 3.66E-05 1.44E-03 1.44E-03 -9.1E-03 -2.66E-03
GWP-luluc kg CO 2 eq 2.87E-02 1.59E-03 9.54E-08 0 7.96E-04 4.16E-05 5.81E-06 7.9E-04 7.9E-04 -4.03E-04 -9E-04
kg CFC11
ODP 2.86E-10 1.71E-14 3.02E-15 0 8.56E-15 7.49E-13 5.34E-14 1.01E-12 1.01E-12 -1.79E-11 -4.39E-11
eq
AP mol H+ eq 3.49E-01 2.72E-04 6.58E-06 0 1.36E-04 3.05E-03 3.6E-05 3.04E-03 3.04E-03 -2.91E-02 -3.19E-02
EP-
kg P eq 1.02E-04 8.53E-07 8.16E-10 0 4.26E-07 2.53E-07 3.98E-08 7.26E-07 7.26E-07 -5.82E-06 -4.91E-06
freshwater
EP-marine kg N eq 1.03E-01 8.47E-05 2.21E-06 0 4.23E-05 1.41E-03 1.27E-05 7.76E-04 7.76E-04 -5.34E-03 -6.34E-03
EP-terrestrial mol N eq 1.2E+00 1.02E-03 3.05E-05 0 5.09E-04 1.66E-02 1.74E-04 8.53E-03 8.53E-03 -4.86E-02 -5.88E-02
kg NMVOC
POCP 2.88E-01 2.37E-04 5.94E-06 0 1.18E-04 3.63E-03 3.41E-05 2.36E-03 2.36E-03 -2.05E-02 -2.67E-02
eq
ADPE kg Sb eq 2.71E-04 2.39E-08 7.39E-11 0 1.19E-08 1.94E-08 1.25E-09 4.39E-08 4.39E-08 -2.64E-05 -2.7E-05
ADPF MJ 1.14E+03 3.82E+00 8.3E-03 0 1.91E+00 2.06E+00 9.88E-02 5.61E+00 5.61E+00 -1.54E+02 -2.32E+02
m3 world eq
WDP 7E+00 2.56E-03 4.01E-03 0 1.28E-03 7.06E-01 2.93E-02 4.7E-02 4.7E-02 -2.47E+00 -2.33E+00
deprived
GWP = Global warming potential; ODP = Depletion potential of the stratospheric ozone layer; AP = Acidification potential of land and water; EP =
Eutrophication potential; POCP = Formation potential of tropospheric ozone photochemical oxidants; ADPE = Abiotic depletion potential for non-fossil
resources; ADPF = Abiotic depletion potential for fossil resources; WDP = Water (user) deprivation potential)
RESULTS OF THE LCA - INDICATORS TO DESCRIBE RESOURCE USE according to EN 15804+A2: 1 m2 Janisol Arte 66
window (47.69 kg/m2)
Parameter Unit A1-A3 A4 A5 C1 C2 C3/1 C3/2 C4/1 C4/2 D/1 D/2
PERE MJ 1.6E+02 2.17E-01 2.91E-01 0 1.08E-01 4.35E-01 3.24E-02 8.42E-01 8.42E-01 -7.37E+00 -1.72E-01
PERM MJ 2.89E-01 0 -2.89E-01 0 0 0 0 0 0 0 0
PERT MJ 1.6E+02 2.17E-01 1.91E-03 0 1.08E-01 4.35E-01 3.24E-02 8.42E-01 8.42E-01 -7.37E+00 -1.72E-01
PENRE MJ 1.04E+03 3.83E+00 8.79E-02 0 1.91E+00 1.03E+02 1.01E+02 5.62E+00 5.62E+00 -1.55E+02 -2.32E+02
PENRM MJ 1.01E+02 0 -7.96E-02 0 0 -1.01E+02 -1.01E+02 0 0 0 0
PENRT MJ 1.14E+03 3.83E+00 8.3E-03 0 1.91E+00 2.06E+00 9.88E-02 5.62E+00 5.62E+00 -1.55E+02 -2.32E+02
SM kg 9.54E+00 0 0 0 0 0 0 0 0 6.79E+00 8.37E+00
RSF MJ 0 0 0 0 0 0 0 0 0 0 0
NRSF MJ 0 0 0 0 0 0 0 0 0 0 0
FW m3 2.82E-01 2.45E-04 9.42E-05 0 1.23E-04 1.66E-02 6.61E-04 1.43E-03 1.43E-03 -6.45E-02 -7.22E-02
5 Environmental Product Declaration - Jansen AG - Janisol Arte 66 window width x height: 1230mm x 1480mm
PERE = Use of renewable primary energy excluding renewable primary energy resources used as raw materials; PERM = Use of renewable primary
energy resources used as raw materials; PERT = Total use of renewable primary energy resources; PENRE = Use of non-renewable primary energy
excluding non-renewable primary energy resources used as raw materials; PENRM = Use of non-renewable primary energy resources used as raw
materials; PENRT = Total use of non-renewable primary energy resources; SM = Use of secondary material; RSF = Use of renewable secondary fuels;
NRSF = Use of non-renewable secondary fuels; FW = Use of net fresh water
RESULTS OF THE LCA – WASTE CATEGORIES AND OUTPUT FLOWS according to EN 15804+A2:
1 m2 Janisol Arte 66 window (47.69 kg/m2)
Parameter Unit A1-A3 A4 A5 C1 C2 C3/1 C3/2 C4/1 C4/2 D/1 D/2
HWD kg 6.18E-07 1.83E-11 8.12E-13 0 9.16E-12 2.34E-10 6.39E-12 2.88E-10 2.88E-10 -2.37E-09 -2.63E-07
NHWD kg 4.86E+00 5.48E-04 5.32E-04 0 2.74E-04 2.63E-01 1.81E-02 2.87E+01 2.87E+01 1.57E+00 1.64E+00
RWD kg 3.26E-02 4.71E-06 4.74E-07 0 2.36E-06 8.94E-05 6.93E-06 6.25E-05 6.25E-05 -3.79E-03 -5.65E-04
CRU kg 0 0 0 0 0 0 0 0 0 0 0
MFR kg 4.29E-01 0 0 0 0 1.59E+01 1.9E+01 0 0 0 0
MER kg 0 0 0 0 0 0 0 0 0 0 0
EEE MJ 0 0 4.02E-02 0 0 1.22E+01 1.59E-01 0 0 0 0
EET MJ 0 0 7.19E-02 0 0 2.19E+01 3.32E-01 0 0 0 0
HWD = Hazardous waste disposed; NHWD = Non-hazardous waste disposed; RWD = Radioactive waste disposed; CRU = Components for re-use;
MFR = Materials for recycling; MER = Materials for energy recovery; EEE = Exported electrical energy; EET = Exported thermal energy
RESULTS OF THE LCA – additional impact categories according to EN 15804+A2-optional:
1 m2 Janisol Arte 66 window (47.69 kg/m2)
Parameter Unit A1-A3 A4 A5 C1 C2 C3/1 C3/2 C4/1 C4/2 D/1 D/2
Disease
PM 2.74E-06 1.64E-09 3.46E-11 0 8.22E-10 1.23E-08 8.9E-10 3.74E-08 3.74E-08 -3.87E-07 -4.01E-07
incidence
IR kBq U235 eq 5.19E+00 6.91E-04 7.71E-05 0 3.45E-04 1.34E-02 8.32E-04 6.95E-03 6.95E-03 -3.91E-01 2.04E-01
ETP-fw CTUe 1.77E+03 2.65E+00 3.81E-03 0 1.33E+00 1.03E+00 7.24E-02 3.14E+00 3.14E+00 -1.7E+01 -6.79E+01
HTP-c CTUh 9.06E-08 5.34E-11 2.5E-13 0 2.67E-11 6.11E-11 2.3E-12 4.8E-10 4.8E-10 -5.21E-09 -6.24E-09
HTP-nc CTUh 3.65E-06 2.76E-09 9.41E-12 0 1.38E-09 3.23E-09 8.74E-11 5.31E-08 5.31E-08 -1.79E-07 -2.28E-07
SQP SQP 2.11E+02 1.31E+00 2.41E-03 0 6.57E-01 4.88E-01 3.5E-02 1.17E+00 1.17E+00 -6.74E+00 -3.51E+00
PM = Potential incidence of disease due to PM emissions; IR = Potential Human exposure efficiency relative to U235; ETP-fw = Potential comparative
Toxic Unit for ecosystems; HTP-c = Potential comparative Toxic Unit for humans (cancerogenic); HTP-nc = Potential comparative Toxic Unit for humans
(not cancerogenic); SQP = Potential soil quality index
Disclaimer 1 – for the indicator 'Potential Human exposure efficiency relative to U235'.This impact category deals mainly with the
eventual impact of low dose ionizing radiation on human health of the nuclear fuel cycle. It does not consider effects due to possible
nuclear accidents, occupational exposure nor due to radioactive waste disposal in underground facilities. Potential ionizing radiation
from the soil, from radon and from some construction materials is also not measured by this indicator.
Disclaimer 2 – for the indicators 'abiotic depletion potential for non-fossil resources', 'abiotic depletion potential for fossil resources',
'water (user) deprivation potential, deprivation-weighted water consumption', 'potential comparative toxic unit for ecosystems', 'potential
comparative toxic unit for humans – cancerogenic', 'Potential comparative toxic unit for humans - not cancerogenic', 'potential soil
quality index'. The results of this environmental impact indicator shall be used with care as the uncertainties on these results are high
or as there is limited experienced with the indicator. This EPD was created using a software tool.
References
Standards EN 12207: 2016 Windows and doors - Air permeability -
Classification
EN 14351-1
EN 14351-1: 2016, Windows and doors - Product standard, EN 13115
performance characteristics - Part 1: windows and external EN 13115: 2020 Windows - Classification of mechanical
pedestrian doorsets properties - Racking, torsion and operating forces
EN 12210
EN 12210: 2016 Windows and doors - Resistance to wind
loads - classification EN 13049
EN 13049 2003 Windows - Soft and heavy body impact - Test
method, safety requirements and classification
EN ISO 10140
EN ISO 10140-1: 2021 Acoustics - Laboratory measurement of EN 15804
sound insulation of building elements - Part 1: Application rules EN 15804:2012+A2:2019+AC:2021, Sustainability of
for specific products construction works — Environmental Product Declarations —
Core rules for the product category of construction products.
DIN EN ISO 10077 ISO 14025
DIN EN ISO 10077-2: 2017 Thermal performance of windows, EN ISO 14025:2011, Environmental labels and declarations —
doors and shutters - Calculation of thermal transmittance - Part Type III environmental declarations — Principles and
2: Numerical method for frames procedures.
ECHA candidate list
EN 12207 ECHA candidate list [BSJ1] - Substances of Very High Concern
– SVHC (date 17.01.2023)
6 Environmental Product Declaration - Jansen AG - Janisol Arte 66 window width x height: 1230mm x 1480mm
Candidate List of substances of very high concern for software.com/international/software/gabi-envision/, 2022
Authorisation (published in accordance with Article 59(10) of
the REACH Regulation) Jansen LCA tool
LCA tool for façades, windows & door
REGULATION (EU) No 528/2012 LCA-Tool No.: IBU-JAN-202301-LT1-EN
REGULATION (EU) No 528/2012 OF THE EUROPEAN Developed by Sphera Solutions GmbH
PARLIAMENT AND OF THE COUNCIL
of 22 May 2012, concerning the making available on the market IBU 2021
and use of biocidal products Institut
Bauen und Umwelt e.V.: General Instructions for the EPD
SBR 2011 programme of Institut Bauen und Umwelt e.V., Version 2.0,
SBR life cycle guide [SBR 2011] Berlin: Institut Bauen und Umwelt e.V., 2021
www.ibu-epd.com
Further References
PCR Part A
Sphera LCA FE Software (GaBi ts) PCR - Part A: Calculation rules for the Life Cycle Assessment
GaBi ts dataset documentation for the software-system and and Requirements on the Background Report, version 1.3,
databases, LBP, University of Stuttgart and thinkstep, Institut Bauen und Umwelt e.V., 2021.
Leinfelden-Echterdingen, 2023 (https://www.gabi-
software.com/support/gabi) PCR Part B
PCR – Part B: Requirements on the EPD for Windows and
Sphera LCA Calculator Software (GaBi Envision) doors, version 1.6, Institut Bauen und Umwelt e.V., www.bau-
GaBi Envision 5.0 Sphera Solution GmbH, the LCA, EPD and umwelt.com, 2022
Ecodesign tool, http://www.gabi-
7 Environmental Product Declaration - Jansen AG - Janisol Arte 66 window width x height: 1230mm x 1480mm
Publisher
Institut Bauen und Umwelt e.V. +49 (0)30 3087748- 0
Hegelplatz 1 info@ibu-epd.com
10117 Berlin www.ibu-epd.com
Germany
Programme holder
Institut Bauen und Umwelt e.V. +49 (0)30 3087748- 0
Hegelplatz 1 info@ibu-epd.com
10117 Berlin www.ibu-epd.com
Germany
Author of the Life Cycle Assessment
Sphera Solutions GmbH +49 711 341817-0
Hauptstraße 111- 113 info@sphera.com
70771 Leinfelden-Echterdingen www.sphera.com
Germany
Owner of the Declaration
JANSEN AG 0041717639113
Industriestrasse 34 sustainability@jansen.com
9463 Oberriet www.jansen.com
Switzerland
8 Environmental Product Declaration - Jansen AG - Janisol Arte 66 window width x height: 1230mm x 1480mm
