ENVIRONMENTAL PRODUCT DECLARATION
as per ISO 14025 and EN 15804+A2
Owner of the Declaration Unilin B.V. Division Panels
Publisher Institut Bauen und Umwelt e.V. (IBU)
Programme holder Institut Bauen und Umwelt e.V. (IBU)
Declaration number EPD-UNI-20230381-IBJ1-EN
Issue date 31.10.2023
Valid to 30.10.2028
Unilin Clicwall
Unilin B.V. Division Panels
www.ibu-epd.com | https://epd-online.com
1. General Information
Unilin B.V. Division Panels Unilin Clicwall
Programme holder Owner of the declaration
IBU – Institut Bauen und Umwelt e.V. Unilin B.V. Division Panels
Hegelplatz 1 Ooigemstraat 3
10117 Berlin 8710 Wielsbeke
Germany Belgium
Declaration number Declared product / declared unit
EPD-UNI-20230381-IBJ1-EN 1 m² of Unilin Clicwall (7.81 kg/m²)
This declaration is based on the product category rules: Scope:
Wood-based panels, 01.08.2021 The scope of this EPD extends to Unilin's Clicwall range. The declared
(PCR checked and approved by the SVR) values refer to the sales-weighted average product. These Clicwall
products are manufactured in the following sites:
Issue date Raw board
31.10.2023 • Bazeilles, France
• Vielsalm, Belgium
Valid to Clicwall board
30.10.2028 • SPANO, Oostrozebeke, Belgium
• BOSPAN, Wielsbeke, Belgium
The owner of the declaration shall be liable for the underlying information
and evidence; the IBU shall not be liable with respect to manufacturer
information, life cycle assessment data and evidences.
The EPD was created according to the specifications of EN 15804+A2. In
the following, the standard will be simplified as EN 15804.
Verification
The standard EN 15804 serves as the core PCR
Dipl.-Ing. Hans Peters
Independent verification of the declaration and data according to ISO
(Chairman of Institut Bauen und Umwelt e.V.)
14025:2011
internally X externally
Florian Pronold Mr Olivier Muller,
(Managing Director Institut Bauen und Umwelt e.V.) (Independent verifier)
1 Environmental Product Declaration - Unilin B.V. Division Panels - Unilin Clicwall
2. Product
requirements apply to the core board (i.e. LF range).
2.1 Product description/Product definition
Unilin Clicwall consists of a raw fiberboard that is pressed with The Clicwall FR is suited for applications where increased fire
an impregnated paper, both on the product's front and protection is required.
backside. The decor on the panel is obtained by applying a
printed decor paper on the raw board. The texture is pressed 2.3 Technical Data
into the melamine surface under high pressure and high Technical characteristics vary by product variant and thickness.
temperature using a special press plate technology. More detailed product-specific data, technical data sheets and
the CE declaration of performance are available on
The fiberboard is available with different compositions (moisture www.unilinpanels.com.
resistant, fire retardant, …) and in different sizes. The surface
Constructional and surface data
does not require further treatment and can be applied in all
The table below summarizes the technical performance of
types of interior projects. The decorative board is durable,
Unilin's Clicwall product for some parameters. The values
scratch resistant, colorfast and easy to maintain. More than 130
below apply to the product range. Performances can depend on
designs are available in Unilin's Decorative range (e.g. woods,
the core board type. Please check the specific "Declaration Of
plain colors and materials).
Performance" of the products available on
www.unilinpanels.com. Specific properties of the declared
Each panel has a tongue on one long side and a groove on the
sales-weighted product are available in 3.10.
other long side, enabling them to click into one another. This
creates a virtually seamless joint on the basis of the Unilin Name Value Unit
patented Uniclic system. The top and bottom are finished flat. Grammage @ 10 mm (EN
7.81 kg/m²
323)
For the placing on the market of the product in the European Bending strength (EN
Depends on core board N/mm²
Union/European Free Trade Association (EU/EFTA) (with the 310)
exception of Switzerland) Regulation (EU) No. 305/2011 (CPR)
E-modulus (EN 310) Depends on core board N/mm²
applies. The product needs a declaration of performance
Thermal conductivity (EN
according: 0.13 W/(mK)
13986)
• EN 13986:2004+A1:2015, Wood-based panels for use
Sound absorption 250 to
in construction – Characteristics, valuation of conformity 0.10
500 HZ (EN 13986)
and marking
Sound absorption 1000 to
• EN 14322:2021, Wood-based panels - Melamine faced 0.20
2000 HZ (EN 13986)
boards for interior uses - Definition, requirements and
classification E1(*); E0.5 (**);
• EN 622-5:2010, Fibreboards - Specifications - Part 5: Formaldehyde CARB/TSCA Title VI (***);
Requirements for dry process boards (MDF) F**** (****)
Surface Soundness (EN
> 1 N/mm²
For the application and use the respective national provisions 311)
apply. Thickness tolerance (EN
± 0.3 mm
324)
The results in this EPD refer to the environmental impact of a
Different formaldehyde emission standards are available
Clicwall product with a sales-weighted average. The
(*) E1 - According to EN 13986+A1:2015 :
composition and thickness of this board was obtained by
averaging the composition of Unilin's entire Clicwall portfolio • a limit value of 0.1 ppm may not be exceeded by EN
based on the annual sales volumes. The declared impact is 717-1 emission chamber method OR
thus representative for the following commercial references at • a limit value of 8 mg HCHO/100 g according to ISO
thicknesses 10 - 12 mm: 12460-5
• Clicwall (LF) (Paint)
(**) E0.5 - According to the ChemVerbotsV :
• Clicwall MR (Black) (Paint)
• Clicwall FR (Uncoloured) (Paint) • a limit value of 0.1 ppm according to EN 16516 OR
• a limit value of 0.05 ppm according to EN 717-1
The values for specific commercial references and thicknesses
can vary from the declared ones. Please contact Unilin's sales (***) CARB 2/TSCA Title VI - According to California Air
team or info.panels@unilin.com for more information. Resources Board & the US Toxic Substances Control Act
(TSCA Title VI) :
2.2 Application
• a limit value of 0.09 ppm according to ASTM E1333 or
Unilin Clicwall is commonly used for interior furniture and
ASTM D6007
decorative interior design in both residential and commercial
projects. Target segments are retail, office, hotel and modular (****) F**** - According to Japanese standard JIS A 5908
construction. The main applications for the panel are listed • a limit value of 0.3 mg/L according to JIS A 1460
below: desiccator
• Seperation walls
• Wall linings Performance data are consistent with the product's declaration
• Ceilings (following specific instructions) of performance with respect to its essential characteristics
All Clicwall products demonstrate low formaldehyde emissions according to:
(since the core board is coated). For some national regulations • EN 13986:2004+A1:2015, Wood-based panels for use
(like CARB2, TSCA Title VI) specific low emissions in construction – Characteristics, valuation of conformity
2 Environmental Product Declaration - Unilin B.V. Division Panels - Unilin Clicwall
and marking
• EN 14322:2021, Wood-based panels - Melamine faced 2.6 Manufacture
boards for interior uses - Definition, requirements and Raw board
classification 1. Round wood is collected to produce the fiberboards.
• EN 622-5:2010, Fibreboards - Specifications - Part 5: 2. The bark is removed from the round wood logs.
Requirements for dry process boards (MDF) 3. The logs are chopped to wood chips.
4. The wood chips are defibrated under high pressure in a
2.4 Delivery status
refiner.
Unilin's Clicwall boards are available in a diverse range of
5. The board is produced by introducing the fibermat into a
dimensions. The most common ones are given below:
press, which compresses it under higher pressure and
• Standard gross dimension: 2785 x 618 x 10 mm (H x W temperature.
x D) 6. The board is sanded, cut into panels and finished
• Standard net dimension: 2785 x 600 x 10 mm (H x W x depending on the intended application.
D)
• High panel gross dimension: 3500 x 618 x 10 mm (H x Clicwall board
W x D)
1. The raw decor paper is impregnated with an
• High panel net dimension: 3500 x 600 x 10 mm (H x W
urea/melamine formaldehyde resin.
x D)
2. The impregnated paper is dried, cut to the correct size
and stacked on pallets or rolls.
Please contact Unilin's sales team or info.panels@unilin.com
3. The press plates, which contain the required surface
for more information on available dimensions of specific
finish, are placed into the melamine press facing the
products.
front- as well as the backside of the panel. The
impregnated paper is positioned on both sides of the
2.5 Base materials/Ancillary materials
raw board.
The data below details the sales-weighted average composition
4. The hot press closes for certain amount of time, during
of Unilin Clicwall.
which the resin bonds the decor paper to the raw board.
5. The panel undergoes an additional quality check and is
Compostion raw board
removed if necessary.
The raw MDF board has a density of 752 kg/m³ and consists of
6. After cooling down, the melamine faced board is cut into
fresh wood, (melamine) urea formaldehyde ((M)UF) glue,
the correct Clicwall dimensions.
additives and moisture. The additives added depend heavily on
7. The Uniclic profile is milled into the decorative MDF
the specific commercial reference (e.g. wax emulsion, fire
board.
retardant based on inorganic salts).
Name Value Unit 2.7 Environment and health during manufacturing
Fresh wood 80 % Unilin's plant management policy is fully integrated in the daily
Glue 11 % operation and governance of its production plants. The aim is to
adhere to legal requirements, minimize negative environmental
Additives 3 %
effects on its neighbors, co-workers and surroundings, and
Moisture 6 %
constantly improve environmental performance. The Bazeilles
The fresh wood is 100% recovered wood, predominantly plant is ISO 9001 and ISO 50001 certified. The Vielsalm site is
sourced from sustainable forest management activities and certified under ISO 9001, ISO 14001 and ISO 45001. The
sawmills (residues & co-products), and mainly consists of BOSPAN and SPANO plants have achieved the ISO 9001
spruce, beech and birch. certificate.
Composition Clicwall board (10 mm) The implementation of Unilin's One Home Sustainability
The sales-weighted average product has a grammage of 7.81 Strategy and its Zero Harm Safety Policy have further set clear
kg/m² and thickness of 10 mm. It consists of a raw MDF board targets to among others reduce the carbon footprint of its
and 2 impregnated decor paper layers, covering the front and production activities, improve the overall resource efficiency
back of the core board. The decor papers are impregnated with and enhance the safety and well-being at its production sites.
an urea/melamine formaldehyde resin to ensure adhesion to
2.8 Product processing/Installation
the surface of the raw board. This impregnated decor paper has
a sales-weighted average grammage of 173 g/m². The Clicwall boards easily click into each other thanks to their
Unilclic profile. This further accommodates a dust-free
The Clicwall board thus has the following composition: installation and delivers an immediately finished result, allowing
the room to be used right after installation. With an impact-
• Raw board: 96 %
resistant and low-maintenance surface, Clicwall also proves
• Impregnated decor paper (front + back): 4 %
durable and easy to care for finish during use. Specific
installation guidelines can be found under
The composition of specific commercial references and
https://www.unilinpanels.com/en/clicwall-wall-cladding/clicwall-
thicknesses can differ from the values depicted above and can
installation.
be obtained by reaching out to info.panels@unilin.com.
Clicwall can be processed (e.g. sawing, milling, drilling) using
Unilin's decorative fiberboard contains Substances of Very High
common utility tools and machinery. It is advised to wear a dust
Concern (SVHCs) or Category 1A or 1B CMR-substances (as
mask when those tools are used without dust extraction. More
defined by ECHA) above 0.1 % by weight: NoThe board further
specific processing and health information is available at
contains no biocides as defined under the EU Biocidal Products
www.unilinpanels.com.
Ordinance No. 528/2012 nor are the boards treated with such
substances. 2.9 Packaging
Product packaging is used to protect the product from damage
during transport. Wood-based chipboards, cardboard, stretch
3 Environmental Product Declaration - Unilin B.V. Division Panels - Unilin Clicwall
foil and PET packaging straps are used as packaging materials. Water
Clicwall does not contain substances that may potentially
2.10 Condition of use contaminate water through leaching. However, it is important, to
The product's composition remains unchanged during its use ensure that the product is not subjected to continuous exposure
and is therefore the same as stated in section 2.5. The glue, to moisture. Prolonged contact with water may result in the
resin and additives are permanently bonded to the wood and degradation of the product.
paper through an irreversible curing process.
Mechanical destruction
2.11 Environment and health during use
When subjected to mechanical stress, the product displays a
Based on current knowledge, using Unilin Clicwall as intended tendency towards brittleness. This could result in the formation
poses no risks to health, water, air or soil. Small amounts of of splinters and sharp broken edges, which may pose a risk of
natural wood constituents could potentially be released, but injury.
aside from negligible amounts of formaldehyde, no harmful
emissions have been detected. 2.14 Re-use phase
Reuse/Recycling
2.12 Reference service life
When a building or furniture has reached its end-of-life phase,
The reference service life (RSL) of the product depends Clicwall can easily be abstracted and collected if selective
significantly on its application. Please contact Unilin's sales dismantling/sorting takes place. After collection, the end-of-life
team or info.panels@unilin.com for more specific information fiberboard can be reused for the same (or different) purpose if
on the product's lifespan in a given set of conditions. possible.
The RSL of Clicwall can vary from 10 to 50 years depending on Energy Recovery
its field of use; according to the BBSR table "BNB In line with the cascading use of wood-based products, the
Nutzungsdauern von Bauteilen (2017)". reuse of the end-of-life Clicwall should be prioritized. However,
if this is not feasible, the board can be used as a secondary fuel
2.13 Extraordinary effects
in approved energy power plants. Its relatively high calorific
Fire
value enables power plants to effectively produce renewable
The fire resistance of Unilin Clicwall depends heavily on its
heat and electricity.
chemical composition (i.e. presence of fire retardants). The
products have the following fire behavior (according to 2.15 Disposal
EN13501-1): Jobsite and post-consumer Clicwall waste (e.g. from demolition
projects) should be reused/recycled where possible, in line with
CE AVCP Class 4 : the cascade principle. Should this not be possible, the waste
• Clicwall (LF): D-s2,d0 (≥ 9 mm/ Bulk density > 600 must be utilized for energy recovery as opposed to being
kg/m³) landfilled (in accordance with EWC waste codes
• Clicwall MR (Black): D-s2,d0 (≥ 9 mm/ Bulk density > 170201/030105).
600 kg/m³)
CE AVCP Class 1 : Waste from packaging materials, which protect the product
from damage during transport, can be reused and recycled if
• Clicwall FR (Uncoloured): B-s2,d0 (10 mm)
sorted correctly.
• Clicwall FR (Uncoloured): B-s1,d0 (12 mm)
2.16 Further information
Fire reaction classes are part of the CE Declaration of
Please contact Unilin's sales team or reach out to
Performance available on Unilin Panels' website
info.panels@unilin.com for additional information.
www.unilinpanels.com.
3. LCA: Calculation rules
3.1 Declared Unit 3.2 System boundary
The declared information and values refer to 1 m² of Unilin This is a cradle-to-gate EPD with options, including the
Clicwall with a sales-weighted average composition, grammage following life cycle phases A1 - A3, C1 - C4 and D. The
of 7.81 kg/m² and thickness of 10 mm. following processes have been considered for each of the
modules:
Declared unit and mass reference
Name Value Unit
A1 - A3: Product Stage
Declared unit 1 m2 The production stage encompasses the extraction of raw
Grammage 7.81 kg/m2 materials (i.e. wood, paper, glue, resin, additives), their
transportation to the production plants, and the subsequent
Layer thickness 0.01 m
manufacturing of the product. The required energy for
This EPD reports the environmental impact of Unilin Clicwall. Its production, ancillary materials, and production emissions are
composition was calculated by averaging Unilin's entire Clicwall included. Energy and material input/output data were obtained
portfolio, using the annual sales volumes as the weighting from Unilin's Bazeilles, Vielsalm, SPANO and BOSPAN plants
factor. The raw board is manufactured at the Bazeilles and as well as its glue factory.
Vielsalm plants. The Clicwall board is produced at the SPANO
and BOSPAN sites. All of these production facilities are in the A large share of the supplied production energy consists of
scope of this declaration. renewable energy, derived from non-recyclable woody waste
streams. These waste streams are sourced in- and externally.
Unilin's fiberboard plants generate renewable thermal energy
on-site. The biomass plants, A&S and A&U, produce renewable
4 Environmental Product Declaration - Unilin B.V. Division Panels - Unilin Clicwall
energy from these woody waste streams, which is directly reported) data. As such, all processes, materials, or emissions
supplied to the SPANO and BOSPAN plants. Any remaining expected to have a significant contribution to the environmental
energy needs are met through the local grid in Belgium or impact of the system under study were considered in the LCA.
France. The total sum of omitted flows can therefore be deemed as
significantly below the 5 % threshold of the system's energy
C1: Deconstruction/Demolition stage and mass input, as stated in the EN 15804+A2.
It is assumed that end-of-life Clicwall is manually dismantled
from the building/furniture. The efforts involved in this process 3.5 Background data
are considered negligible, leading to the absence of a declared The relevant background data was either taken from the
environmental impact arising from the dismantling of the EcoInvent 3.8. database or peer-reviewed literature sources.
product. Measures were taken to ensure that the used secondary data
was no more than 10 years old. These data types allowed to
C2: Transport to Waste Processing map the background system in the LCA of the product under
This life cycle stage describes the impact of the end-of-life study.
product's transport from the demolition site to the waste
3.6 Data quality
processing facility. A representative distance of 50 km is
assumed. Data collection and necessary calculations were done in line
with ISO 14044. Primary data was directly gathered from the
C3: Waste Processing designated person at the relevant production plants. It was
Processing of post-consumer Clicwall waste involves ensured that the collected data accurately represented reality,
(preliminary) sorting and shredding of the material. The so it can be assumed that the used primary data is of high
fiberboard is repurposed as a secondary fuel and undergoes quality.
energy recovery in module D. The material and its inherent
properties (e.g. biogenic carbon and primary energy content) The technological, geographical, and time-related
are thus exported from the system in C3. representativeness of background data (e.g. from EcoInvent)
was verified, as stated in EN 15804+A2.
C4: Waste Disposal
3.7 Period under review
This module describes the loads and emissions attributed to
Primary data, needed to calculate the LCA of the system under
the disposal of the product after waste processing. As the end-
study, was collected for the year 2020 from the Bazeilles,
of-life product leaves the system in C3 as a secondary fuel, no
Vielsalm, BOSPAN, SPANO and Unilin's glue production facility.
environmental impact is declared in C4.
3.8 Geographic Representativeness
D: Loads and Benefits beyond the System Boundaries
Land or region, in which the declared product system is
Module D describes the loads and benefits related to the use of
manufactured, used or handled at the end of the product´s
the end-of-life Clicwall as a secondary fuel. This involves the
lifespan: Western Europe
energy recovery of post-consumer fiberboard waste, where it
replaces a European-averaged mix of electricity and heat.
3.9 Allocation
The system boundary between subsequent systems is defined In line with EN 15804+A2 and EN 16485, the biogenic carbon
in accordance with EN 15804+A2, i.e. when the material and primary energy content of the wood have been balanced
reaches its end-of-waste state. The end-of-life product reaches over the product's entire life cycle (A1 - C4) based on its
its end-of-waste state after a sorting and shredding step, as inherent material characteristics and underlying physical flows.
inventoried in C3. The material leaves the current system at Fresh wood inventories were taken from EcoIvent 3.8. Here, it
module C3 and enters a subsequent system as a secondary was made sure that the biogenic carbon and energy content
fuel. reflect the physical relationships of the different wood-based
materials.
3.3 Estimates and assumptions
Specific, primary data have been used to the highest extent
The system boundary (and subsequent allocation) relating to
possible. In case of absence, estimates and assumptions were
the flow of the end-of-life product are as described in section
made to model reality as closely as possible. These
3.2.
assumptions are based on publicly available data and literature.
Generic dataset from the EcoInvent 3.8. database have been 3.10 Comparability
used to model the impact of some raw materials and process- Basically, a comparison or an evaluation of EPD data is only
related parameters for which specific data was lacking. possible if all the data sets to be compared were created
according to EN 15804 and the building context, respectively
End-of-life Clicwall leaves the product system in C3 as a the product-specific characteristics of performance, are taken
secondary fuel, for which the benefits and loads are inventoried into account. Background data was used from the EcoInvent
in module D. Here it is assumed that the secondary fuel 3.8. database.
substitutes electricity and heat in accordance with an average
mix available on the European grid.
3.4 Cut-off criteria
All in- and outputs to the system under study have been
included in the LCA. Primary data was used to the highest
extent possible. If primary data was lacking, secondary data
from EcoInvent was resorted to. Conservative assumptions
were made using average or generic data in case of data gaps.
These assumptions are based on publicly available (literature
5 Environmental Product Declaration - Unilin B.V. Division Panels - Unilin Clicwall
4. LCA: Scenarios and additional technical information
info.panels@unilin.com for more information.
Characteristic product properties of biogenic carbon
End-of-life (C1-C4)
The values declared below describe the amount of biogenic
The following table provides the parameters required to model
carbon and stored biogenic CO in the building product under
2 the end-of-life of the product under study. Since the product is
study when it leaves the factory gate. These relate to 1 m² of
not intended for extended outdoor use, it is assumed that its
Unilin Clicwall, with a sales-weighted average composition and
moisture content remains consistent with its state at the factory
thickness (i.e. 10 mm).
gate. The end-of-life product reaches its end-of-waste state
Biogenic carbon content at factory gate after (preliminary) sorting and shredding. The losses during the
The carbon uptake of the packaging materials is not included sorting and shredding are assumed to have a negligible impact
below as their end-of-life impact is not declared in module A5. and are thus discarded. The material leaves the system as a
secondary fuel (energy recovery).
Name Value Unit
Biogenic carbon content in product 3.0 kg C/m² Name Value Unit
Stored carbon dioxide in product 11.0 kg CO2/m² Collected separately 7.81 kg/m²
Secondary fuel (output at C3) 7.81 kg/m²
Note: 1 kg biogenic carbon is equivalent to 44/12 kg CO .
2
Reuse, recovery and/or recycling potentials (D)
In module D, the loads and benefits of exporting the secondary
The following technical information is a basis for the declared
fuel from the system under study are inventoried. The moisture
modules or can be used for developing specific scenarios in the
content of this fuel is assumed to remain consistent with its
context of a building assessment if modules are not declared
state at factory gate. This value may vary significantly based on
(MND).
the storage conditions prior to its intended use.
Installation into the building (A5)
The end-of-life impact of the used packaging materials is not The recovery potential is modelled based on the net output flow
declared. However, its impact can be modelled based on the of secondary fuel. It is assumed that a biomass power plant
data given below. located in the EU recovers the secondary fuel's energy, with 55
% of the energy being recovered as heat and the remaining 30
Name Value Unit
% as electricity. The generated energy carriers are assumed to
Wood-based packaging 0.42 kg/m²
substitute heat and electricity in accordance with the average
Cardboard 0.0041 kg/m² mix available on the European grid.
PET straps 0.0036 kg/m² Name Value Unit
Stretch foil 0.00058 kg/m² Net output flow of secondary fuel 7.01 kg/m²
Information on the reference lifetime can be found in section Energy efficiency biomass plant 85 %
2.12. Please contact Unilin's sales team or
6 Environmental Product Declaration - Unilin B.V. Division Panels - Unilin Clicwall
5. LCA: Results
The values declared below refer to 1 m² of Unilin Clicwall with a sales-weighted average composition, grammage of 7.81 kg/m² and
thickness of 10 mm.
Table "Description of the system boundary" summarizes the scope of the system under study from a life cycle point of view. Declared
modules are indicated with an "X", non-declared modules are indicated with "MND". "MNR" refers to modules which are deemed as not
relevant.
DESCRIPTION OF THE SYSTEM BOUNDARY (X = INCLUDED IN LCA; MND = MODULE OR INDICATOR NOT DECLARED; MNR
= MODULE NOT RELEVANT)
Benefits and
Construction loads beyond
Product stage Use stage End of life stage
process stage the system
boundaries
la ire ta m w a Ry lp p u s tro p s n a rT g n iru tc a fu n a M e h t m o rf tro p s n a rTe tis e h t o t e ta g y lb m e s s A e s U e c n a n e tn ia M ria p e R tn e m e c a lp e R tn e m h s ib ru fe R y g re n e la n o ita re p Oe s u re ta w la n o ita re p Oe s u n o itc u rts n o c -e Dn o itilo m e d tro p s n a rT g n is s e c o rp e ts a W la s o p s iD -e s u e R-y re v o c e R-g n ilc y c e Rla itn e to p
A1 A2 A3 A4 A5 B1 B2 B3 B4 B5 B6 B7 C1 C2 C3 C4 D
X X X MND MND MND MND MNR MNR MNR MND MND X X X X X
RESULTS OF THE LCA - ENVIRONMENTAL IMPACT according to EN 15804+A2: 1 m² Unilin Clicwall
Parameter Unit A1-A3 C1 C2 C3 C4 D
Global Warming Potential total (GWP-total) kg CO 2 eq -7.68E+00 0 3.52E-02 1.11E+01 0 -5.96E+00
Global Warming Potential fossil fuels (GWP-fossil) kg CO 2 eq 3.23E+00 0 3.51E-02 1.32E-01 0 -5.94E+00
Global Warming Potential biogenic (GWP-biogenic) kg CO 2 eq -1.09E+01 0 1.09E-05 1.1E+01 0 -1.29E-02
Global Warming Potential luluc (GWP-luluc) kg CO 2 eq 1.56E-02 0 1.3E-05 1.79E-04 0 -9.59E-03
Depletion potential of the stratospheric ozone layer (ODP) kg CFC11 eq 5.95E-07 0 8.46E-09 1.89E-08 0 -8.96E-07
Acidification potential of land and water (AP) mol H+ eq 2.25E-02 0 1.48E-04 7.42E-04 0 -8.9E-03
Eutrophication potential aquatic freshwater (EP-freshwater) kg P eq 1.9E-04 0 2.42E-07 7.24E-06 0 -4.22E-04
Eutrophication potential aquatic marine (EP-marine) kg N eq 6.22E-03 0 4.47E-05 1.89E-04 0 4.29E-03
Eutrophication potential terrestrial (EP-terrestrial) mol N eq 6.81E-02 0 4.93E-04 2.11E-03 0 4.62E-02
Formation potential of tropospheric ozone photochemical oxidants kg NMVOC
2.36E-02 0 1.59E-04 5.99E-04 0 8.3E-03
(POCP) eq
Abiotic depletion potential for non fossil resources (ADPE) kg Sb eq 3.63E-05 0 8.39E-08 4.39E-07 0 -1.98E-06
Abiotic depletion potential for fossil resources (ADPF) MJ 8.62E+01 0 5.52E-01 2.39E+00 0 -1.66E+02
m3 world eq
Water use (WDP) 3.9E+00 0 1.87E-03 6.63E-03 0 -9E-01
deprived
RESULTS OF THE LCA - INDICATORS TO DESCRIBE RESOURCE USE according to EN 15804+A2: 1 m² Unilin Clicwall
Parameter Unit A1-A3 C1 C2 C3 C4 D
Renewable primary energy as energy carrier (PERE) MJ 6.87E+01 0 7.03E-03 1.15E+02 0 -1.37E+01
Renewable primary energy resources as material utilization
MJ 1.14E+02 0 0 -1.15E+02 0 0
(PERM)
Total use of renewable primary energy resources (PERT) MJ 1.83E+02 0 7.03E-03 2.53E-01 0 -1.37E+01
Non renewable primary energy as energy carrier (PENRE) MJ 6.29E+01 0 5.52E-01 2.53E+01 0 -1.66E+02
Non renewable primary energy as material utilization (PENRM) MJ 2.36E+01 0 0 -2.29E+01 0 0
Total use of non renewable primary energy resources (PENRT) MJ 8.65E+01 0 5.52E-01 2.39E+00 0 -1.66E+02
Use of secondary material (SM) kg 2.27E-03 0 0 0 0 0
Use of renewable secondary fuels (RSF) MJ 6.35E+00 0 0 0 0 8.76E+01
Use of non renewable secondary fuels (NRSF) MJ 0 0 0 0 0 1.75E+01
Use of net fresh water (FW) m3 1.08E-01 0 6.57E-05 1.33E-03 0 -6.68E-02
RESULTS OF THE LCA – WASTE CATEGORIES AND OUTPUT FLOWS according to EN 15804+A2:
1 m² Unilin Clicwall
Parameter Unit A1-A3 C1 C2 C3 C4 D
Hazardous waste disposed (HWD) kg 1.73E-01 0 3.82E-04 3.56E-03 0 -7.28E-03
Non hazardous waste disposed (NHWD) kg 2.42E+00 0 5.45E-02 9.77E-02 0 -1E+00
Radioactive waste disposed (RWD) kg 4.64E-04 0 3.74E-06 1.67E-05 0 -6.59E-04
Components for re-use (CRU) kg 0 0 0 0 0 0
Materials for recycling (MFR) kg 0 0 0 0 0 0
Materials for energy recovery (MER) kg 0 0 0 7.81E+00 0 0
Exported electrical energy (EEE) MJ 0 0 0 0 0 0
Exported thermal energy (EET) MJ 0 0 0 0 0 0
RESULTS OF THE LCA – additional impact categories according to EN 15804+A2-optional:
1 m² Unilin Clicwall
7 Environmental Product Declaration - Unilin B.V. Division Panels - Unilin Clicwall
Parameter Unit A1-A3 C1 C2 C3 C4 D
Disease
Incidence of disease due to PM emissions (PM) 2.5E-07 0 4.17E-09 8.74E-09 0 8.88E-08
incidence
Human exposure efficiency relative to U235 (IR) kBq U235 eq 3.64E-01 0 2.4E-03 1.63E-02 0 -7.59E-01
Comparative toxic unit for ecosystems (ETP-fw) CTUe 2.06E-05 0 6.77E-10 3.32E-09 0 -1.49E-08
Comparative toxic unit for humans (carcinogenic) (HTP-c) CTUh 1.91E-08 0 5.66E-12 3.7E-11 0 4.24E-10
Comparative toxic unit for humans (noncarcinogenic) (HTP-nc) CTUh 2.2E-09 0 1.72E-11 1.22E-10 0 -7.54E-10
Soil quality index (SQP) SQP 7.72E+02 0 6.32E-01 1.16E+00 0 -1.29E+01
Disclaimer 1 – for the indicator 'Potential Human exposure efficiency relative to U235'. This impact category deals mainly with the
eventual impact of low-dose ionizing radiation on human health of the nuclear fuel cycle. It does not consider effects due to possible
nuclear accidents, occupational exposure or radioactive waste disposal in underground facilities. Potential ionizing radiation from the
soil, radon and from some construction materials is also not measured by this indicator.
Disclaimer 2 – for the indicators 'abiotic depletion potential for non-fossil resources', 'abiotic depletion potential for fossil resources',
'water (user) deprivation potential, deprivation-weighted water consumption', 'potential comparative toxic unit for ecosystems', 'potential
comparative toxic unit for humans – cancerogenic', 'Potential comparative toxic unit for humans - not cancerogenic', 'potential soil
quality index'. The results of this environmental impact indicator shall be used with care as the uncertainties on these results are high
as there is limited experience with the indicator.
6. LCA: Interpretation
This section aims to analyze and interpret the results of the high wood content (i.e. 77 %) results in a GWP-total of - 7.7
LCA analysis carried for 1 m² of Unilin Clicwall. The results kg/m². The product thus stores carbon and does not contribute
shown below refer to the product with a sales-weighted to global warming when it leaves the Unilin's factory gate. The
average composition and thickness (10 mm). Although the stored carbon will only be released if the Clicwall board can no
values for specific commercial references and thicknesses can longer fulfill its intended purpose (i.e. at end of life).
vary from the declared and discussed ones, the observed
trends will be the same throughout the entire product category. A deep dive in the drivers of the cradle-to-gate environmental
impact shows the significant contribution of the raw materials
Summary (module A1). 71 % of the fossil CO emissions can primarily be
2
This part intends to summarize the trends observed in the allocated to the glue and resin production, as well as 93 % of
cradle-to-gate environmental impact of Clicwall. An in-depth the water used in A1 - A3. The generation of heat and
analysis is available in the following subsections. electricity, required for the Clicwall production, is an important
driver of the production-related impact. This is observable in the
During its growth, wood absorbs CO 2 through photosynthesis EP and POCP indicators.
and stores it as biogenic carbon in its biomass. The product's
when Clicwall leaves the factory gate. The product under study
Cradle-to-Cradle Impact - Dominance Analysis thus stores carbon and does not contribute to global warming.
The hot-spot analysis highlights the negative GWP-value of
modules A1 - A3, as depicted in the GWP-focused graph. To The stored carbon will only be released when the product
improve the clarity of the graph, the values of the GWP-luluc leaves the system as a secondary fuel. The figure below clearly
indicator have been omitted. demonstrates a neutral biogenic carbon balance in accordance
with EN 16485.
Wood stores CO as biogenic carbon during its growth (GWP-
2
biogenic = - 11 kg CO eq./m²). This negative GWP-value is The GWP-focused analysis also illustrates the "avoided" impact
2
(described in module D) related to the export of end-of-life
partially counterbalanced by the positive GWP-impact of the
Clicwall as a secondary fuel. The energy recovery of that fuel
fossil materials and energy resources used during A1 - A3
generates heat and electricity, which substitutes a European-
(GWP-fossil). This results in a GWP-total of - 7.7 kg CO eq./m²
2
8 Environmental Product Declaration - Unilin B.V. Division Panels - Unilin Clicwall
averaged mix of heat and electricity from the grid. Since the The hot-spot analysis shows that, for non-GWP-related
largest share of the heat and electricity on the European grid is parameters, modules A1 - A3 are the main contributors to the
fossil-based, a negative GWP-fossil is obtained (i.e. avoided system under study. Values for module D are generally
fossil CO emissions from combustion). It indicates that the negative, except for the EP and POCP indicators. This is
2
combustion of these fossil fuels has a higher impact on global attributed to the emissions from the energy recovery process of
warming than the energy recovery from the secondary fuel. the end-of-life fiberboard.
Cradle-to-Grave Impact - Main Drivers indicators ADPE and WDP. 93 % of all water used in modules
The graph below allows to identify the primary sources of the A1 - A3 is allocated to the production of the raw materials
cradle-to-gate environmental impact. The results show that raw (mainly related to the glue and resin production).
material production (module A1) has a significant impact. 71 %
of the fossil CO emissions are primarily attributed to the Energy-related processes are typically the main drivers of the
2
production of the used glue and resin. The contribution of the environmental impact of module A3. This is observed in the
raw material production is even more significant for the contribution of A3 to EP and POCP, which is traced back to the
generation of renewable energy from woody waste.
9 Environmental Product Declaration - Unilin B.V. Division Panels - Unilin Clicwall
7. Requisite evidence
Formaldehyde emissions
AFFSET - Arrêté du 19 avril 2011 (28 days [Class])
E1 - EN 13986:2004+A1:2015 • Test Report : 402-21-1109C-3-f-e
• Method : ISO 16000
• Test report : 1110
• Product : Clicwall
• Method : EN 717-1
• Laboratory : FCBA
• Product : Clicwall
• Laboratory : TCNH
Name Value Unit
• Result : 0.01 ppm [Limit < 0.1 ppm]
Formaldehyde A+ Class
E0.5 - ChemVerbotsV Acetaldehyde A+ Class
Toluene A+ Class
• Test report : 1110
• Method : EN 717-1 Tetrachloroethylene A+ Class
• Product : Melamine Faced MDF Xylene A+ Class
• Laboratory : Clicwall 1,2,3- Trimethylbenzene A+ Class
• Result : 0.01 ppm [Limit < 0.05 ppm]
1,4-dichlorobenzene A+ Class
Ethylbenzene A+ Class
2-Butoxyethanol A+ Class
PCP + Heavy metals + Wood preservative analysis
Styrene A+ Class
As Unilin Melamine faced fibreboard does not contain any post- COVT fid A+ Class
consumer recycled wood, this evidence is not necessary.
VOC Emissions
Melamine faced fiberboards are commonly used for interior
building. In many countries national regulations are applicable
for indoor air quality. For other indoor air analysis reports
please contact Unilin's sales team or info.panels@unilin.com
for more information.
German AgBB (2021) overview of results (28 days [µg/m³])
• Test Report : ML01911-10R
• Method : ISO 16516
• Product : Melamine Faced Fibromax (= Clicwall)
• Laboratory : Servaco Product Testing
Name Value Unit
TVOC (C6 - C16) < 1000 μg/m3
Sum SVOC (C16 - C22) < 100 μg/m3
R (dimensionless) < 1 -
VOC without NIK < 100 μg/m3
Carcinogenic Substances < 1 μg/m3
10 Environmental Product Declaration - Unilin B.V. Division Panels - Unilin Clicwall
8. References
Standards
EN 13986
ASTM D6007
EN 13986:2004+A1:2015, Wood-based panels for use in
ASTM D6007:2020, Standard Test Method for Determining construction— Characteristics, valuation of conformity and
Formaldehyde Concentrations in Air from Wood Products Using marking
a Small-Scale Chamber.
EN 14322
ASTM E1333
EN 14322:2021, Wood-based panels - Melamine faced boards
ASTM E1333:2020, Standard Test Method for Determining for interior uses - Definition, requirements and classification.
Formaldehyde Concentrations in Air and Emission Rates from
Wood Products Using a Large Chamber. EN 15804
EN 310 EN 15804:2012+A2:2019+AC:2021, Sustainability of
construction works — Environmental Product Declarations —
EN 310:1993, Wood-based panels - Determination of modulus Core rules for the product category of construction products.
of elasticity in bending and of bending strength.
EN 16000 - 3
EN 311
EN 16000 - 3: 2011, Air sampting on DNPH cartidge and
EN 311:2002, Wood-based panels - Surface soundness - Test analysis of Iow molecularweight carbonyl compounds by
method. HPLC/UV
EN 319 EN 16000 - 6
EN 319:1993, Particleboards and fibreboards - Determination EN 16000 - 6: 2012, Air sampling on multiadsorbent (Tenax TA /
of tensile strength perpendicular to the plane of the board. gtass wool) and analysis of volatile organic compounds (VOC)
by TD/cCmS/FID
EN 322
EN 16000 - 9
EN 322:1993, Wood-based panels - Determination of moisture
content. EN 16000 - 9: 2006, lndoor air - Paft 9: Determination of the
emission of volatile organic compounds from building products
EN 323 and furnishing - Emission test chamber method
EN 323:2005, Wood-based panels - Determination of density. EN 16000 - 11
EN 324 EN 16000 - 11: 2006, Indoor air — Part 11: Determination of the
emission of volatile organic compounds from building products
EN 324-1:1993, Wood-based panels - Determination of and furnishing — Sampling, storage of samples and
dimensions of boards - Part 1: Determination of thickness, preparation of test specimens.
width and length.
EN 16449
EN 622
EN 16449:2014, Wood and wood-based produts - Calculation
EN 622-5:2010, Fibreboards - Specifications - Part 5: of the biogenic carbon content of wood and conversion to
Requirements for dry process boards (MDF). carbon dioxide.
EN 717-1 EN 16485
EN 717-1:2004, Wood-based panels - Determination of EN 16485:2014, Round and sawn timber. Environmental
formaldehyde release Formaldehyde emission by the chamber Product Declarations. Product category rules for wood and
method. wood-based products for use in construction.
EN 12460-5 EN 16516
EN 12460-5:2015, Wood-based panels. Determination of EN 16516:2020, Construction products: Assessment of release
formaldehyde release Extraction method (called the perforator of dangerous substances - Determination of emissions into
method). indoor air.
EN 13501-1 ISO 9001
EN 13501-1:2007-05+A1:2009, Fire classification of EN ISO 9001:2008-11, Quality Management Systems –
construction products and building elements - Part 1: Requirements
classification with the results of tests on the reaction to fire of
building products.
11 Environmental Product Declaration - Unilin B.V. Division Panels - Unilin Clicwall
ISO 14001 and Council of 9th March 2011 to define harmonized conditions
for marketing building products.
EN ISO 14001:2015, Environmental management systems —
Requirements with guidance for use. EcoInvent 3.8.
ISO 14025 Ecoinvent 3.8, Database for Life Cycle Inventory and
Assessment. Swiss Centre for Life Cycle Inventories, 2021.
EN ISO 14025:2011, Environmental labels and declarations — Available at: https://ecoinvent.org/the-ecoinvent-database/data-
Type III environmental declarations — Principles and releases/ecoinvent-3-8/.
procedures.
EU Biocidal Products Ordinance No. 528/2012
ISO 14040
Regulation (EU) No 528/2012 of the European Parliament and
EN ISO 14040:2006-10, Environmental management — Life Council of 22 May 2012 concerning the making available on the
cycle assessment — Principles and framework. market and use of biocidal products.
ISO 14044 EWC
ISO 14044:2006-10, Environmental management — Life cycle European Waste Catalogue, Ordinance on the European Waste
assessment — Principles and framework. Catalogue (Waste Catalogue Ordinance - AVV), reference
Federal Official Journal I 2001, 3379.
ISO 45001
IBU 2022
EN ISO 45001:2018, Occupational health and safety
management systems — Requirements with guidance for use. Institut Bauen und Umwelt e.V.: General Instructions for the
EPD programme of Institut Bauen und Umwelt e.V., Version
ISO 50001 2.1, Berlin: Institut Bauen und Umwelt e.V., 2022
www.ibu-epd.com
EN ISO 50001:2018, Energy management systems —
Requirements with guidance for use. PCR Part A
JIS A 1460 Product Category Rules for Building-Related Products and
Services. Part A: Calculation Rules for the Life Cycle
JIS A 1460:2021, Building boards Determination of Assessment and Requirements on the Project Report according
formaldehyde emission -- Desiccator method. to EN 15804+A2:2019. Version 1.3. Berlin: Institut Bauen und
JIS A 5908 Umwelt e.V. (eds.), 2021.
JIS A 5908:2022, Particleboards. PCR Part B
Additional References Product Category Rules for Building-Related Products and
Services. Part B: Requirements on the EPD for Wood based
BBSR Table panels. Version 2. Berlin: Institut Bauen und Umwelt e.V. (eds.),
2023.
BBSR 2017, Useful lives of building components for life cycle
analyses according to the Sustainable Building Assessment SVHC List
System, 2017, BBSR Germany 2017.
List of Substances of Very High Concern (SVHC) Candidate for
CPR Authorisation (ECHA Candidate List), dated 04.07.2023,
published in accordance with Article 59(10) of the REACH
CPR EU Ordinance No. 305/2011 of the European Parliament Regulation. Helsinki: European Chemicals Agency.
12 Environmental Product Declaration - Unilin B.V. Division Panels - Unilin Clicwall
Publisher
Institut Bauen und Umwelt e.V. +49 (0)30 3087748- 0
Hegelplatz 1 info@ibu-epd.com
10117 Berlin www.ibu-epd.com
Germany
Programme holder
Institut Bauen und Umwelt e.V. +49 (0)30 3087748- 0
Hegelplatz 1 info@ibu-epd.com
10117 Berlin www.ibu-epd.com
Germany
Author of the Life Cycle Assessment
Unilin B.V. Division Panels +32 56 67 52 11
Ooigemstraat 3 info.panels@unilin.com
8710 Wielsbeke https://www.unilinpanels.com/en-
Belgium gb
Owner of the Declaration
Unilin B.V. Division Panels +32 56 66 70 21
Ooigemstraat 3 info.panels@unilin.com
8710 Wielsbeke https://www.unilinpanels.com/en-
Belgium gb
13 Environmental Product Declaration - Unilin B.V. Division Panels - Unilin Clicwall
