ENVIRONMENTAL PRODUCT DECLARATION
as per ISO 14025 and EN 15804+A2
Owner of the Declaration Swisspearl Group AG
Publisher Institut Bauen und Umwelt e.V. (IBU)
Programme holder Institut Bauen und Umwelt e.V. (IBU)
Declaration number EPD-SWP-20230359-CCA1-EN
Issue date 24.10.2023
Valid to 23.10.2028
Corrugated Sheets
Swisspearl Group AG
www.ibu-epd.com | https://epd-online.com
General Information
Swisspearl Group AG Corrugated Sheets
Programme holder Owner of the declaration
IBU – Institut Bauen und Umwelt e.V. Swisspearl Group AG
Hegelplatz 1 Eternitstrasse 3
10117 Berlin 8867 Niederurnen
Germany Switzerland
Declaration number Declared product / declared unit
EPD-SWP-20230359-CCA1-EN 1m2 of fibre cement Corrugated sheets
This declaration is based on the product category rules: Scope:
Fibre cement / Fibre concrete, 01.08.2021 This EPD refers to fibre cement corrugated sheets on behalf of Swisspearl
(PCR checked and approved by the SVR) Group AG, produced in the factories located in Trzemeszno (Poland) and
Šumperk (Czech Republic) and are based on the production volumes of
the year 2021.
Issue date The owner of the declaration shall be liable for the underlying information
and evidence; the IBU shall not be liable with respect to manufacturer
24.10.2023
information, life cycle assessment data and evidences.
The EPD was created according to the specifications of EN 15804+A2. In
Valid to
the following, the standard will be simplified as EN 15804.
23.10.2028
Verification
The standard EN 15804 serves as the core PCR
Independent verification of the declaration and data according to ISO
14025:2011
internally X externally
Dipl.-Ing. Hans Peters
(Chairman of Institut Bauen und Umwelt e.V.)
Florian Pronold Dr. Matthew Fishwick,
(Managing Director Institut Bauen und Umwelt e.V.) (Independent verifier)
1 Environmental Product Declaration - Swisspearl Group AG - Corrugated Sheets
Product
The main constituents of the Swisspearl Corrugated sheets are
Product description/Product definition as followed:
Swisspearl Corrugated sheets are used as roofing material on
• Portland cement (grey): 70-85%
wooden or metal sub construction. This declaration is based on
• Inert filler (limestone, mica, silica): 5-15%
the average of the various types of Corrugated sheets
• Cellulose: 3-8%
produced both in Trzemeszno (Poland) and Šumperk (Czech
• Polyvinyl alcohol (PVA): 0-2%
Republic). These include the product names: W130, W146,
• Paint: 0-2%
W172, W177, coated and uncoated, and with reinforcing
Material explanation
possibilities. Swisspearl Corrugated sheets are available in
6mm and 6,5mm thicknesses. For the placing on the market of • Portland Cement: Manufactured according to
the product in the European Union/European Free Trade /DIN EN 197-1/ from limestone, marl and
Association (EU/EFTA) (with the exception of Switzerland) sand. The material is crushed, dried,
Regulation (EU) No. 305/2011 (CPR) applies. The product calcinated to clinker and ground to cement.
needs a declaration of performance taking into consideration • Inert filler: a filler to optimize deformation
EN 494:2012+A1 'Fibre-cement profiled sheets and fittings - properties and material bonding.
Product specification and test methods' and the CE-marking. • Cellulose Fibres (0.5-3mm): To assure
collection of powder during filtration.
Application • PVA fibres (4-6mm): Synthetic Polyvinyl alcohol fibre
Swisspearl Corrugated sheets are intended for installation used as reinforcement.
as roofing and/or cladding on wooden or metal sub There are no substances of very high concern (SVHC) present
constructions in the product according to according to Regulation (EC) No.
1907/2006 (REACH).
Technical Data
The technical specifications of Swisspearl Corrugated sheets Manufacturing
can be seen in the following table: Swisspearl Corrugated sheets are manufactured with
Constructional data Hatschek technology at both factories.
A very thin slurry of water, binder and fibres is mixed
Name Value Unit
and introduced into each of the vats of the Hatschek
Thermal conductivity 0.4 W/(mK)
machine. The rotating sieve cylinder in the vats
Gross density dry min 1600 kg/m3 collects a thin layer of solid material that is further
Moisture content at 23 °C, 80% dewatered as it is transferred to a felt and further on to
11 M.-%
humidity an accumulating format roller. At the required
thickness, the accumulated layers are automatically
Coefficient of thermal expansion 10 10-6K-1
cut into the required product size, corrugated, and
Min.
Min. breaking load N/m transferred into the pre-curing area, and waste is
4250
returned to the manufacturing process. After pre-curing, the
Min. breaking moment Min. 55 NM/m products are stored under continued control
Water vapour permeability 10 mmHg*hr*m2/g of temperature and humidity. Swisspearl Corrugated
Moisture expansion 0 mm/m sheets are delivered in natural grey and coated
versions in various colours with a smooth and even
Further information can be found in the Download Center on
surface. The backside has an anti-blocking treatment.
the Swisspearl website
Reference service life
Product according to the CPR, based on a hEN]: Performance The current type of Swisspearl Corrugated sheets was
data of the product in accordance with the Declaration of introduced in the beginning of the 2000s. There are therefore
Performance (DoP) with respect to its essential characteristics no substantiated data on the reference service life (RSL).
according to EN 494:2012+A1 'Fibre-cement profiled sheets However, it is estimated that the RSL of Swisspearl Corrugated
and fittings - Product specification and test methods' and the sheets is 50 years or higher. This is in accordance with the
CE-marking. table published by the Bundesinstitut für Bau-, Stadt- und
Raumforschung (BBSR) (code 335.511), which estimates the
Base materials/Ancillary materials
RSL of facade and roofing products produced from fibrecement.
LCA: Calculation rules
Name Value Unit
Declared Unit
Declared Unit 1 m2
In this EPD the declared unit is defined as the production of
1m2 of Swisspearl Corrugated sheets, with an expected lifetime Gross density ,dry min 1600 kg/m3
of 50 years or higher, and its related impacts over the 'cradle to Layer thickness 0.006 m
grave' life-cycle modules. Grammage 14 kg/m2
The EPD results are based on 1m2 of corrugated sheets with a
thickness of 6mm, however Swisspearl Corrugated sheets are
Data from production sites
also available in thicknesses of 6,5mm. In order to obtain the
Data is gathered for the production process of at the factory
EPD results for 6,5 mm sheets, the results need to be multiplied
sites in Poland and Czech Republic for the year 2021.
by 1,085 (conversion factor).
This EPD quantifies the average environmental impact of the
Declared unit and mass reference different corrugated sheets variants produced in these factories
2 Environmental Product Declaration - Swisspearl Group AG - Corrugated Sheets
(W130, W146, W172, W177), including coated and uncoated be reusable over time, but this is not included in this
versions. assessment. Incineration credits for the packaging material
The average is calculated by collecting all production data per have been considered.
declared unit of product and weigh them based on their
production volume. Differences between the product variants Background data and data quality
are considered to be small. Modelling of the production of 1m2 of Swisspearl Corrugated
sheets is done with GaBi Software System and Database for
Life Cycle Engineering. The model has been developed by
Sphera Solutions GmbH. Each background dataset has been
System boundary
reviewed on geographical, technological, and temporal scale.
The modules considered in this EPD follow a cradle to grave
assessment: A1-A5, B1-B7, C1-C4, D. Technological: All primary and secondary data are modelled to
A1 -The system boundaries include the provision and be specific to the technology mixes under study. Proxy data are
processing of raw materials. These include in particular cement, used where technology-specific data are unavailable. The
plastic fibres, pulp and packaging materials. technological representativeness is considered to be good.
A2 -The transports to the manufacturer were specifically Geographical: All primary and secondary data are collected
collected for all starting materials. specific to the countries/regions under study. Where
country/region specific data are unavailable, proxy data are
A3 -The production includes also all in-plant energy used. The geographical representativeness is considered to be
consumption (gas + electricity), as well as water used in the good.
production process, and production waste.
Temporal: All primary data collected is based on the year 2021.
All secondary data come from the GaBi 2020.1 databases and
A4 -The transport, part of the construction process, is an are representative for the years 2020-2025. Temporal
average of the total distance of all products delivered to the representativeness is considered to be very good.
point of installation. This is calculated to be 1964 km.
Allocation in foreground data
A5 -All environmental impacts associated with the disposal of The production process does not deliver any co-products.
packaging handled at the construction site are accounted for. It Therefore, the applied model does not contain any allocation.
is assumed incinerated at an incineration plant. Disposal of
product waste is assumed to be landfilled. Furthermore, Allocation for waste materials
environmental impacts associated with trucks and fuel for the Pre-processing waste (plastics) is sent to a waste incineration
construction installation are included. plant. The resulting electrical and thermal energy is credited in
module A1. For the waste incineration plant an R1-value of
B1-B7 modules are included, however, no significant above 0.6 is assumed.
environmental impact is associated with the use phase of the The resulting credits based on the incineration of the packaging
product. of the product are declared in module D.
C1 -Accounts for the environmental impacts associated with Cut-off criteria
dismantling and demolition of the fibre cement boards. Fuel All raw materials used, utilized thermal energy, and electric
used for demolition equipment and transport on-site vehicles. power consumption of the production process are considered in
this assessment. This means that all material and energy flows
C2 -Transportation of the discarded products from the contributing less than 1% are considered.
construction site to a landfilling site. The transport is estimated
to be 100 km in an average truck. Geographic Representativeness
Land or region, in which the declared product system is
C3 -The fibre cement boards are sent to landfill and therefore manufactured, used or handled at the end of the product´s
there are no environmental impacts associated with waste lifespan: Europe
processing of materials flows intended for reuse, recycling or
energy recovery.
Comparability
C4 -Environmental impacts associated with the processes at Basically, a comparison or an evaluation of EPD data is only
the landfill. possible if all the data sets to be compared were created
according to EN 15804 and the building context, respectively
D -The fibre cement boards are sent to landfill after use. The the product-specific characteristics of performance, are taken
product has therefore no impact during this stage and no into account. GaBi Software System and Database for Life
associated environmental impacts. The boards are expected to Cycle Engineering CUP Version: 2022.2
LCA: Scenarios and additional technical information
Name ValueUnit
Characteristic product properties of biogenic carbon
kg
The biogenic carbon containing material (cellulose) in Biogenic carbon content in product 0.02
C
Swisspearl Corrugated sheets is required to be listed
Biogenic carbon content in accompanying kg
separately. The following table shows the biogenic carbon 0.01
packaging C
content in the product and accompanying packaging:
Information on describing the biogenic Carbon Content at
factury gate Note: 1 kg of biogenic carbon is equivalent to 44/12 kg of CO 2.
3 Environmental Product Declaration - Swisspearl Group AG - Corrugated Sheets
Name Value Unit
Plastic waste 0.008 kg
Transport to the building site (A4) Pallets 0.007 kg
Estimating the transport to each individual construction site is Screws 12 pcs
rather complex. However, an educated estimate is made for the
In case a reference service life according to applicable ISO
distance to the installation point by averaging the total distance
standards is declared then the assumptions and in-use
of all products delivered to Swisspearl's warehouses and
conditions underlying the determined RSL shall be declared. In
adding 100 km, representing the distance from the warehouse
addition, it shall be stated that the RSL applies for the reference
to the installation point. Swisspearl's warehouses for which the
conditions only. The same holds for a service life declared by
distance has been calculated are located in Denmark, Sweden,
the manufacturer. Corresponding information related to in-use
Norway, Netherlands, Belgium, Ireland and the United
conditions needs not be provided if a service life taken from the
Kingdom.
list on service life by BNB is declared.
Name Value Unit
Reference service life
Transport distance 1964 km
Name ValueUnit
Gross density of products transported 1600 kg/m3
Reference service life (according to ISO 15686-1, -
0 - 0 a
Installation into the building (A5) 2, -7 and -8)
Installation of the boards is carried out by use of an Life Span (according to BBSR) >50 a
automatic screwdriver. It is estimated that 12 screws Life Span according to the manufacturer 0 - 0 a
are used for the installation of the declared unit of
Swisspearl Corrugated sheets. End of life (C1-C4)
Name Value Unit
PE film and wooden pallets are used as packaging
Reuse - kg
materials. Polyethylene foils can be recycled locally, and
Landfilling ~14 kg
reusable pallets can be returned to the building
material suppliers.
4 Environmental Product Declaration - Swisspearl Group AG - Corrugated Sheets
LCA: Results
The following tables show the results of life-cycle assessment indicators, resource use and waste related to 1m2 of Swisspearl
Corrugated fibre cement sheets. The data is representative of the products of Swisspearl.
DESCRIPTION OF THE SYSTEM BOUNDARY (X = INCLUDED IN LCA; MND = MODULE OR INDICATOR NOT DECLARED; MNR
= MODULE NOT RELEVANT)
Benefits and
Construction loads beyond
Product stage Use stage End of life stage
process stage the system
boundaries
la ire ta m w a Ry lp p u s tro p s n a rT g n iru tc a fu n a M e h t m o rf tro p s n a rTe tis e h t o t e ta g y lb m e s s A e s U e c n a n e tn ia M ria p e R tn e m e c a lp e R tn e m h s ib ru fe R y g re n e la n o ita re p Oe s u re ta w la n o ita re p Oe s u n o itc u rts n o c -e Dn o itilo m e d tro p s n a rT g n is s e c o rp e ts a W la s o p s iD -e s u e R-y re v o c e R-g n ilc y c e Rla itn e to p
A1 A2 A3 A4 A5 B1 B2 B3 B4 B5 B6 B7 C1 C2 C3 C4 D
X X X X X X X X X X X X X X X X X
RESULTS OF THE LCA - ENVIRONMENTAL IMPACT according to EN 15804+A2: 1 m^2 Swisspearl Corrugated sheets
Parameter Unit A1 A2 A3 A4 A5 B1 B2 B3 B4 B5 B6 B7 C1 C2 C3 C4 D
GWP-total kg CO 2 8.41E 1.37E- 1.61E 1.37E 1.14E 0 0 0 0 0 0 0 3.18E- 6.98E- -2.19E- 1.03E -1.26E-
eq +00 01 +00 +00 +00 04 02 01 +00 01
GWP-fossil kg CO 2 8.39E 1.33E- 1.95E 1.31E 7.78E- 0 0 0 0 0 0 0 3.15E- 6.67E- 6.44E-01 1.66E- -1.26E-
eq +00 01 +00 +00 01 04 02 01 01
GWP- kg CO 2 1.36E- 4.01E- -3.36E- 6.03E- 3.64E- 0 0 0 0 0 0 0 2.68E- 3.07E- -8.65E- 8.67E- -6.08E-
biogenic eq 02 03 01 02 01 06 03 01 01 04
GWP-luluc kg CO 2 2E-03 3.01E- 3.73E-04 3.11E- 5.48E- 0 0 0 0 0 0 0 4.46E- 1.58E- 1.58E-03 4.89E- -8.25E-
eq 06 05 04 07 06 04 05
kg CFC11 1.67E- 1.47E- 5.38E- 7.54E- 7.65E- 6.46E- -1.36E-
ODP 4.25E-15 1.5E-16 0 0 0 0 0 0 0 9.71E-15
eq 14 17 15 18 18 16 15
1.71E- 1.08E- 1.88E- 6.55E- 5.49E- 1.18E-
AP mol H+ eq 1.5E-02 3.77E-03 0 0 0 0 0 0 0 5.47E-03 -1.6E-04
03 03 03 07 05 03
EP- 4.38E- 2.87E- 2.78E- 1.43E- 8.45E- 1.42E- 2.79E- -1.56E-
kg P eq 4.34E-06 0 0 0 0 0 0 0 1.69E-05
freshwater 06 08 07 06 10 08 07 07
5.03E- 4.78E- 3.41E- 1.56E- 1.73E- 3.07E-
EP-marine kg N eq 8.59E-04 4.3E-04 0 0 0 0 0 0 0 1.72E-03 -4.6E-05
03 04 04 07 05 04
5.24E- 3.77E- 4.67E- 1.63E- 1.92E- 3.38E- -4.93E-
EP-terrestrial mol N eq 5.5E-02 9.18E-03 0 0 0 0 0 0 0 1.82E-02
03 03 03 06 04 03 04
kg
1.34E- 1.03E- 1.37E- 4.22E- 5.24E- 9.32E- -1.29E-
POCP NMVOC 1.7E-02 3.89E-03 0 0 0 0 0 0 0 4.9E-03
03 03 03 07 05 04 04
eq
3.39E- 4.42E- 4.58E- 3.91E- 9.26E- 2.33E- 1.57E- -2.01E-
ADPE kg Sb eq 8.16E-08 0 0 0 0 0 0 0 2.12E-07
07 09 08 05 11 09 08 08
5.28E 1.79E 2.13E 1.85E 7.91E 9.44E- 1.02E 2.21E -2.18E
ADPF MJ 0 0 0 0 0 0 0 5.6E-03
+01 +00 +01 +01 +00 01 +01 +00 +00
m3 world
3.01E- 2.14E- 2.17E- 5.63E- 5.05E- 1.11E- 1.79E- -9.13E-
WDP eq 6.89E-02 0 0 0 0 0 0 0 1.3E-02
01 04 03 02 05 04 02 03
deprived
GWP = Global warming potential; ODP = Depletion potential of the stratospheric ozone layer; AP = Acidification potential of land and water; EP =
Eutrophication potential; POCP = Formation potential of tropospheric ozone photochemical oxidants; ADPE = Abiotic depletion potential for non-fossil
resources; ADPF = Abiotic depletion potential for fossil resources; WDP = Water (user) deprivation potential)
RESULTS OF THE LCA - INDICATORS TO DESCRIBE RESOURCE USE according to EN 15804+A2: 1 m^2 Swisspearl
Corrugated sheets
Parameter Unit A1 A2 A3 A4 A5 B1 B2 B3 B4 B5 B6 B7 C1 C2 C3 C4 D
-8.26E- 5.97E- 5.01E 6.11E- 1.76E 2.58E- 3.11E- 2.74E 7.79E -4.68E-
PERE MJ 0 0 0 0 0 0 0
01 03 +00 02 +00 03 03 +01 +00 01
7.49E -7.49E
PERM MJ 0 1.4E-01 0 -1.4E-01 0 0 0 0 0 0 0 0 0 0 0
+00 +00
6.66E 5.97E- 5.15E 6.11E- 1.62E 2.58E- 3.11E- 2.74E 2.97E- -4.68E-
PERT MJ 0 0 0 0 0 0 0
+00 03 +00 02 +00 03 03 +01 01 01
5.28E 1.79E 2.09E 1.86E 8.29E 9.46E- 1.02E 2.21E -2.18E
PENRE MJ 0 0 0 0 0 0 0 5.6E-03
+01 +00 +01 +01 +00 01 +01 +00 +00
PENRM MJ 0 0 3.4E-01 0 -3.4E-01 0 0 0 0 0 0 0 0 0 0 0 0
5.28E 1.79E 2.13E 1.86E 7.95E 9.46E- 1.02E 2.21E -2.18E
PENRT MJ 0 0 0 0 0 0 0 5.6E-03
+01 +00 +01 +01 +00 01 +01 +00 +00
SM kg 1.24E-01 0 0 0 0 0 0 0 0 0 0 0 0 0 0 0 0
RSF MJ 0 0 0 0 0 0 0 0 0 0 0 0 0 0 0 0 0
NRSF MJ 0 0 0 0 0 0 0 0 0 0 0 0 0 0 0 0 0
9.63E- 4.11E- 9.82E- 2.69E- 2.51E- 5.45E- -4.57E-
FW m3 1.73E-02 0 0 0 0 0 0 0 5E-06 7.2E-03
06 03 05 03 06 04 04
5 Environmental Product Declaration - Swisspearl Group AG - Corrugated Sheets
PERE = Use of renewable primary energy excluding renewable primary energy resources used as raw materials; PERM = Use of renewable primary
energy resources used as raw materials; PERT = Total use of renewable primary energy resources; PENRE = Use of non-renewable primary energy
excluding non-renewable primary energy resources used as raw materials; PENRM = Use of non-renewable primary energy resources used as raw
materials; PENRT = Total use of non-renewable primary energy resources; SM = Use of secondary material; RSF = Use of renewable secondary fuels;
NRSF = Use of non-renewable secondary fuels; FW = Use of net fresh water
RESULTS OF THE LCA – WASTE CATEGORIES AND OUTPUT FLOWS according to EN 15804+A2:
1 m^2 Swisspearl Corrugated sheets
Parameter Unit A1 A2 A3 A4 A5 B1 B2 B3 B4 B5 B6 B7 C1 C2 C3 C4 D
6.46E- 1.28E- 3.36E- 1.28E- 1.02E- 1.48E- 8.38E- 2.34E- -4.86E-
HWD kg 0 0 0 0 0 0 0 6.5E-12
09 11 09 10 09 12 09 10 10
4.39E- 1.79E- 4.71E- 1.86E- 1.89E- 3.97E- 9.46E- 3.29E- -9.84E-
NHWD kg 0 0 0 0 0 0 0 1.1E+01
02 04 01 03 02 06 05 02 04
1.47E- 1.94E- 5.17E- 1.99E- 3.08E- 8.34E- 1.01E- 7.32E- 2.32E-
RWD kg 0 0 0 0 0 0 0 -1.5E-04
03 06 04 05 04 07 06 04 05
CRU kg 0 0 0 0 0 0 0 0 0 0 0 0 0 0 0 0 0
MFR kg 0 0 0 0 0 0 0 0 0 0 0 0 0 0 0 0 0
MER kg 0 0 0 0 0 0 0 0 0 0 0 0 0 0 0 0 0
3.82E-
EEE MJ 0 0 0 0 0 0 0 0 0 0 0 0 0 0 0 0
04
2.27E-
EET MJ 0 0 0 0 0 0 0 0 0 0 0 0 0 0 0 0
04
HWD = Hazardous waste disposed; NHWD = Non-hazardous waste disposed; RWD = Radioactive waste disposed; CRU = Components for re-use;
MFR = Materials for recycling; MER = Materials for energy recovery; EEE = Exported electrical energy; EET = Exported thermal energy
RESULTS OF THE LCA – additional impact categories according to EN 15804+A2-optional:
1 m^2 Swisspearl Corrugated sheets
Parameter Unit A1 A2 A3 A4 A5 B1 B2 B3 B4 B5 B6 B7 C1 C2 C3 C4 D
Disease 1.83E- 2.85E- 5.99E- 2.24E- 5.52E- 3.05E- 3.48E- 1.47E- -1.38E-
PM 7.6E-08 0 0 0 0 0 0 0
incidence 07 08 09 08 12 10 07 08 09
kBq U235 2.29E- 2.75E- 4.89E- 2.82E- 3.83E- 1.37E- 1.43E- 1.19E- 2.44E- -2.47E-
IR 0 0 0 0 0 0 0
eq 01 04 02 03 02 04 04 01 03 02
2.35E 6.54E 1.34E 2.18E 2.36E- 6.84E- 6.59E 1.26E -4.34E-
ETP-fw CTUe 1.3E+00 0 0 0 0 0 0 0
+01 +00 +01 +00 03 01 +00 +00 01
1.12E- 2.41E- 1.97E- 6.67E- 1.27E- 3.46E- 1.85E- -2.05E-
HTP-c CTUh 2.5E-10 7.8E-10 0 0 0 0 0 0 0
09 11 10 14 11 10 10 11
1.17E- 1.04E- 1.04E- 9.25E- 2.52E- 5.32E- 2.19E- 2.05E- -8.12E-
HTP-nc CTUh 1.1E-08 0 0 0 0 0 0 0
07 09 08 09 12 10 08 08 10
4.46E 4.63E- 5.25E 4.75E- 1.33E 1.77E- 2.42E- 4.15E 4.46E-
SQP SQP 0 0 0 0 0 0 0 -3.2E-01
+00 03 +01 02 +00 03 03 +02 01
PM = Potential incidence of disease due to PM emissions; IR = Potential Human exposure efficiency relative to U235; ETP-fw = Potential comparative
Toxic Unit for ecosystems; HTP-c = Potential comparative Toxic Unit for humans (cancerogenic); HTP-nc = Potential comparative Toxic Unit for humans
(not cancerogenic); SQP = Potential soil quality index
Disclaimer 1 – for the indicator “Potential Human exposure efficiency relative to U235”. This impact category deals mainly with the
eventual impact of low-dose ionizing radiation on human health of the nuclear fuel cycle. It does not consider effects due to possible
nuclear accidents, occupational exposure or radioactive waste disposal in underground facilities. Potential ionizing radiation from the
soil, radon and from some construction materials is also not measured by this indicator.
Disclaimer 2 – for the indicators “abiotic depletion potential for non-fossil resources”, “abiotic depletion potential for fossil resources”,
“water (user) deprivation potential, deprivation-weighted water consumption”, “potential comparative toxic unit for ecosystems”,
“potential comparative toxic unit for humans – cancerogenic”, “Potential comparative toxic unit for humans - not cancerogenic”,
“potential soil quality index”. The results of this environmental impact indicator shall be used with care as the uncertainties on these
results are high as there is limited experience with the indicator.
This EPD was created using a software tool.
References
Standards ISO 15686-1, -2, -7 and -8
ISO 15686-1:2011
DIN EN 197-1 Part 1 General principles and framework
DIN EN 197-1, Cement - Part 1: Composition, specificationsand Part 2 Service life prediction procedures
conformity criteria for common cements. Part 7 Performance evaluation for feedback of service life data
EN 494 from practice
EN 494:2012+A1, Fibre-cement profiled sheets and fittings — Part 8 Reference service life and service-life estimation
Product specification and test methods.
EN 15804
ISO 14025 EN 15804:2012+A1:2013, Sustainability of construction works
EN ISO 14025:2011, Environmental labels and declarations — — Environmental Product Declarations — Core rules for the
Type III environmental declarations — Principles and product category of construction products.
procedures.
EN 15804
EN 15804:2012+A2:2019+AC:2021, Sustainability of
6 Environmental Product Declaration - Swisspearl Group AG - Corrugated Sheets
construction works — Environmental Product Declarations — EPD programme of Institut Bauen und Umwelt e.V., Version
Core rules for the product category of construction products. 2.0, Berlin: Institut Bauen und Umwelt e.V., 2021 www.ibu-
epd.com
REACH
Regulation (EC) No 1907/2006, Registration, Evaluation, PCR Part A
Authorisation and Restriction of Chemicals (REACH) Calculation Rules for the Life Cycle Assessment and
Requirements on the Project Report,Berlin: Institut Bauen und
Further References Umwelt e.V., www.ibu-epd.com, Version 2.2, 2022
BBSR PCR Part B
Bundesinstitut für Bau-, Stadt- und Raumforschung Requirements of the EPD for Fibre Cement/Fibre Concrete,
(BBSR): Nutzungsdauer von Bauteilen für version 1.7, Institut Bauen und Umwelt e.V., www.bau-
Lebenszyklusanalyse nach Bewertungssystem umwelt.com, 2019
Nachhaltiges Bauen (BNB), 2011
REGULATION (EU) No 305/2011 Harmonised conditions for
GaBi documentation the marketing of construction products and repealing Council
GaBi life cycle inventory data documentation Directive 89/106/EEC
www.gabisoftware.com/support/gabi/gabidatabase2020lcidocumentation
Swisspearl Group A/G
GaBi software Swisspearl Group A/G: Information on technical data and
Sphera Solutions GmbH downloads.
GaBi Software System and Database for Life Cycle Downloads - Swisspearl
Engineering
CUP Version: 2022.2
University of Stuttgart The literature referred to in the Environmental Product
Leinfelden Echterdingen Declaration must be listed in full.Standards already fully quoted
in the EPD do not need to be listed here again.
IBU 2021 The current version of PCR Part A and PCR Part B of the PCR
Institut Bauen und Umwelt e.V.: General Instructions for the document on which they are based must be referenced.
7 Environmental Product Declaration - Swisspearl Group AG - Corrugated Sheets
Publisher
Institut Bauen und Umwelt e.V. +49 (0)30 3087748- 0
Hegelplatz 1 info@ibu-epd.com
10117 Berlin www.ibu-epd.com
Germany
Programme holder
Institut Bauen und Umwelt e.V. +49 (0)30 3087748- 0
Hegelplatz 1 info@ibu-epd.com
10117 Berlin www.ibu-epd.com
Germany
Author of the Life Cycle Assessment
Sphera Solutions GmbH +49 711 341817-0
Hauptstraße 111- 113 info@sphera.com
70771 Leinfelden-Echterdingen www.sphera.com
Germany
Owner of the Declaration
Swisspearl Group AG +41 56 617 11 11
Eternitstrasse 3 info@group.swisspearl.com
8867 Niederurnen www.swisspearl.com
Switzerland
8 Environmental Product Declaration - Swisspearl Group AG - Corrugated Sheets
