ENVIRONMENTAL-PRODUCT DECLARATION
as per ISO 14025 and EN 15804+A1
Owner of the Declaration ROCKWOOL ROCKFON GmbH
Publisher Institut Bauen und Umwelt e.V. (IBU)
Programme holder Institut Bauen und Umwelt e.V. (IBU)
Declaration number EPD-RWI-20200018-CBD1-EN
Issue date 03.05.2023
Valid to 09.03.2025
Ceiling Tiles
ROCKWOOL ROCKFON GmbH
www.ibu-epd.com | https://epd-online.com
General Information
ROCKWOOL ROCKFON GmbH Ceiling Tiles
Programme holder Owner of the declaration
IBU – Institut Bauen und Umwelt e.V. ROCKWOOL ROCKFON GmbH
Hegelplatz 1 Rockwool Straße 37-41
10117 Berlin D-4596 Gladbeck
Germany Germany
Declaration number Declared product / declared unit
EPD-RWI-20200018-CBD1-EN 1 m² of installed ceiling tile.
This declaration is based on the product category rules: Scope:
Mineral panels, 08.03.2023 The span of products covered under this declaration is synthetic resin-
(PCR checked and approved by the SVR) bonded stone wool materials, which are produced in the form of tiles in the
density range from 70 up
to 175kg/m³. The products are supplied in thicknesses of 12 up to 160 mm.
Issue date The
declared product in this declaration is Rockfon Arctic with a density of
03.05.2023
100kg/m3 and a thickness
of 15mm. For the rest of the products scaling factors are provided. For the
facing and coating materials, information can be found in the attached
Valid to
Annex.
09.03.2025 The products included in this EPD are manufactured in Roermond
(Netherlands), Cigacice (Poland), Saint Eloy (France), Vyborg (Russia)
and Marshall County, Mississippi (USA). The EPD is based on weighted
LCA inventory data from the 5 plants.
The owner of the declaration shall be liable for the underlying information
and evidence; the IBU shall not be liable with respect to manufacturer
information, life cycle assessment data and evidences.
The EPD was created according to the specifications of EN 15804+A1. In
the following, the standard will be simplified as EN 15804 bezeichnet.
Verification
Dipl.-Ing Hans Peters
The standard EN 15804 serves as the core PCR
(chairman of Institut Bauen und Umwelt e.V.)
Independent verification of the declaration and data according to ISO
14025:2011
internally X externally
Dipl.-Ing. Hans Peters Dr. Frank Werner,
(Managing Director Institut Bauen und Umwelt e.V.) (Independent verifier)
1 Environmental-Product Declaration - ROCKWOOL ROCKFON GmbH - Ceiling Tiles
Product
The acoustic tiles can have a glass fibre fleece facing and
Product description/Product definition can be coated with water-based dispersion paint. Details for the
Rockfon environmental impacts of this type of facing can be found on
stone wool acoustic tiles are traditionally made from volcanic the first page of the annex. The additional
rock (typically facing of aluminium laminate may be applicable for some
basalt or dolomite), an increasing proportion of recycled products. The environmental impacts of aluminium laminate are
material, and a low presented on the second page of the annex. Product-specific
percentage of binder (in Rockfon acoustic tiles this is around 3- environmental impacts are compiled by applying the relevant
4%). The scaling factor (listed in the table below) in the Product Specific
essential component of Rockfon tiles are stone wool fibres, Scaling formula.
which are monofilament Product Specific Scaling Formula:
synthetic mineral fibres of non-crystalline structure extracted Environmental Impact per m2 product X-with facing =
from a silicate Environmental Impact reference product*scaling factor
melt. The products described in this EPD are produced in the +Environmental Impact facing material.
form of tiles in Please note that the scaling factors give the precise amount of
the density range from 70 up to 175 kg/m³. The products are material needed to produce the other product types.
supplied in thicknesses
of 12 up to 160 mm.
2 Environmental-Product Declaration - ROCKWOOL ROCKFON GmbH - Ceiling Tiles
For the Name Value Unit
placing on the market of the product in the European Gross density 70 - 175 kg/m3
Union/European Free Trade
Reaction to Fire acc. to EN 13964 A1
Association (EU/EFTA) (with the exception of Switzerland)
Regulation (EU) No. Sound absorption coefficient (αw)
up to 1.00
305/2011 (CPR) applies. The product needs a declaration of acc. to EN 13964
performance taking Susceptibility to the growth of
into consideration EN harmful micro-organisms, as A - not susceptible
13964:2014 or EN 13162+A1:2015 and the CE-marking. dampness acc. to EN 13964
For Thermal conductivity acc. to EN
0.04 W/mK
the application and use the respective national provisions apply. 13964
They meet the requirements of the regulation (EU)
Susceptibility to the growth of
Nr. 1272/2008/EU.
harmful micro-organisms, through A
thermal insulation acc. to EN 13964
Application
Durability acc. to EN 13964 Class 1/C/0N
Rockfon
products include acoustic ceiling tiles, baffles, islands and wall Sound absorption class A
applications. They are available with different coatings and Light reflection up to 87% %
facings in a Light diffusion up to >99% %
variety of shapes, thicknesses, and densities and positively
up to 100% RH
contribute to a healthy indoor environment.
Humidity and sag resistance and no visible %
Technical Data deflection
The technical specifications listed below cover the range of all Airborne sound reduction acc. to EN
up to 42 dB
the products declared in this EPD. For information regarding ISO 10848-2 and EN ISO 717-1
specific products please visit https://www.rockfon.co.uk and Performance
access the provided Declarations of Performance (DoP). data of the Rockfon stone wool products are in accordance with
Constructional data (acc. to EN 13964) the declaration
of performance with respect to its essential characteristics
according to EN 13964:2014.
Emission tests according to
EN 16516:2018 are available from national technical managers.
Base materials/Ancillary materials
Composition
Rockfon stone wool product:
• non-scarce natural stone and cement [59%]
• slags and other secondary materials or waste materials
[19,5%]
• mineral oil and bonding agent [<0,2%]
• binder, a thermoset inert polymer resin [5%]
• Non-woven glass wool facing (optional) [1-15%]
3 Environmental-Product Declaration - ROCKWOOL ROCKFON GmbH - Ceiling Tiles
• water-based paints [0-16,5%] BBSR table. According to this table, mineral panels have a
Packaging represents less than 6% of the final product service life of more than 50 years in a building. For this EPD the
delivered to the customer. The raw materials are non-scarce declared value is therefore 50 years.
natural stones, secondary materials and briquettes, which are
made of mineral wool waste, secondary materials and by- This
products from other industries such as slags and cement. The is the service life that is used in most existing PCRs and EPDs
binder is a thermoset inert polymer resin which is polymerized in the Dutch,
into a solid resin during the production of the final stone wool German, US and Canadian markets. The mineral wool core in
product. The coating is a waterborne acrylic coating and an Rockfon
additional (optional) polyurethane (PU) coating. products is tested to maintain its properties for at least 50
This product/article/at least one partial article years. Also, Rockfon
contains substances listed in the candidate list (ECHA products are tested to maintain flatness even in high
PR/19/12) (date: 16.07.2019) exceeding 0.1 percentage by temperature/ high humidity
mass: no environments (40°C /
Mineral wool fibres produced by ROCKWOOL are classified as 95 % relative humidity). Given this, there is no doubt that
non-hazardous under REACH (Regulation (EC) No 1272/2008 Rockfon ceiling
of the European Parliament and of the council of 16 December tiles could have a technical lifespan of more than 50 years in a
2008 on classification, labelling and packaging of substances normal indoor
and mixtures). environment.
ROCKWOOL stone wool is registered with REACH under the
following definition: “Man-made vitreous (silicate) fibres with
random orientation with alkaline oxide and alkali earth oxide
(Na O+K O+CaO+MgO+BaO) content greater than 18% by
2 2
weight and fulfilling one of the Note Q conditions”. ROCKWOOL Some owners will replace the Rockfon product due to
products produced in Europe fulfil the Note Q requirements. renovations or aesthetics, but not for functional performance
This is certified by the independent certification body EUCEB. reasons.
(European Certification Board for mineral wool products). More Replacements typically do not happen due to technical failure
information on EUCEB can be found under www.euceb.org. but are more
likely the result of vandalism, accidents, visual appearance,
Environment and health during use minor refurbishments (e.g. painting an office, changing of
tenants) or major
Reference service life refurbishments.
A reference service life according to ISO 15686 is not declared
for this EPD. Instead, a service life is declared according to
LCA: Calculation rules
• Transporting the raw materials and preliminary materials
Declared Unit to ROCKWOOL production facilities;
The declared unit refers to 1 m² of installed acoustic • Production process in the ROCKWOOL production
ceiling tile or wall panel (within the density range 70 – 175 facilities including energy inputs and emissions;
kg/m3) with the • Electricity consumption;
results being representative for a 15 mm thick and 1,5 kg/m2 • Waste processing up to the end-of-waste state or
heavy disposal of waste residues, during the production stage;
product. This weight per m2 is applicable for • Production of packaging material;
the stone wool core without the facing. The declared product is • Manufacturing of products and co-product.
Rockfon Arctic The environmental impact of co-products coming for example
with a density of 100kg/m3 and a thickness of 15 mm. from the steel and electricity plants (e.g. slags, alumina and
ashes entering the system as inputs to the manufacturing) is
Declared unit
accounted for and economic allocation is applied.
Name Value Unit Recycled stone wool comes free of environmental burden, as it
Declared unit 1 m2 enters the product system as waste. Its transport to the factory
is accounted for. Modules A1, A2 and A3 are declared as an
Grammage 1.5 kg/m2
aggregated module A1-A3.
Thickness of the panels 15 mm
Layer thickness - m In two of the factories (Cigacice in Poland and Roermond in the
Netherlands) we obtain Renewable Energy Certificates for the
complete electricity consumption. For that purpose the
System boundary electricity in those factories is modelled as renewable electricity.
EPD type: Cradle to gate with options, modules C1–C4, and
module D.
The modules considered in the life cycle assessment as per Construction/Installation
system boundaries are described as follows: The Construction Stage A4-A5 includes:
• A4 transport to the building site
• A5 installation to the building
Production The transport in A4 is modelled based on the amount
The product stage A1-A3 includes: of tiles that fit in a truck that can hold 44 pallets. The values are
• Provision of preliminary products and energy and based on annual average delivery data. In A5 the default
relevant upstream processes; installation is assumed to be manual, therefore no energy
4 Environmental-Product Declaration - ROCKWOOL ROCKFON GmbH - Ceiling Tiles
consumption or ancillary equipment is needed. • B7 – Operational water use:
The product waste from installation is assumed to be 7% and Rockfon stone wool ceiling tiles are installed permanently in the
according to the modularity principle of EN 15804, its impacts structure and do not require maintenance, repair, replacement
are fully allocated to A5. The 7% assumption is used based on or refurbishment under normal use conditions. Similarly,
the "common scenarios for LCA" internal document from Rockfon has no operational energy or water use.
EURIMA (European Insulation Manufacturers Association) but
can, in reality, be significantly lower. End of Life
The A5 stage, The End-of-life stage C1-C4 includes:
according to EN 15804 includes also waste
• C1 de-construction, demolition;
processing up to the end-of-waste state or disposal of
• C2 transport to waste processing;
final residues during the construction process stage
• C3 waste processing for reuse, recovery and/or
and impacts and aspects related to product losses
recycling;
during installation. Finally, the A5
• C4 disposal.
module includes also the corresponding end-of-life
These stages also include the provision and all transport,
considerations for packaging. The assumption for installation
provision of all materials, products and related energy and
waste for this
water use. Manual deconstruction is assumed for C1 and no
calculation is that it is 100% landfilled but it often also is 100%
impacts are assigned. The benefits from disposal (heat or
closed-loop
electricity recovery) are assigned to module D.
recycled through the Rockfon recycling service offering.
Building Use
Module D includes reuse, recovery and/or recycling potentials
The use-stage B1-B7, related to the building fabric
expressed as net loads and benefits. Here the loads from the
includes:
packaging disposal in A5 and from electricity generation on
• B1 use or application of the installed product -not part of landfill are considered.
this EPD;
• B2 maintenance; The product system with the system boundaries is presented in
• B3 repair; the graph below:
• B4 replacement;
• B5 refurbishment;
• B6 – Operational energy use:
Geographic Representativeness Comparability
Land or region, in which the declared product system is Basically, a comparison or an evaluation of EPD data is only
manufactured, used or handled at the end of the product´s possible if all the data sets to be compared were created
lifespan: Global according to EN 15804 and the building context, respectively
the product-specific characteristics of performance, are taken
5 Environmental-Product Declaration - ROCKWOOL ROCKFON GmbH - Ceiling Tiles
into account.
LCA: Scenarios and additional technical information
The following technical information for the declared modules
Reference service life
can be used for scenario development in a building context.
Name Value Unit
Transport to the building site (A4)
Life Span (according to BBSR) > 50 a
Name Value Unit
Litres of fuel 38 l/100km Operational energy use (B6) and Operational water use
(B7)
Transport distance 646 km
Name Value Unit
Capacity utilisation (including empty runs) 85 %
Gross density of products transported 100 kg/m3 Water consumption - m3
Electricity consumption - kWh
Installation into the building (A5) Other energy carriers - MJ
Name Value Unit Equipment output - kW
Electricity consumption - kWh
End of life (C1-C4)
Material loss 7 %
Use or application of the installed product (B1) see section Name Value Unit
2.12 "Use"
Landfilling 15 kg
Name Value Unit
Transport to landfill 50 km
Maintenance (B2) Utilization rate 50 %
Name Value Unit
Information on maintenance - - Reuse, recovery and/or recycling potentials (D), relevant
scenario information
Maintenance cycle - Number/RSL
Any declared benefits and loads from net flows leaving the
Water consumption - m3 product system that have not been allocated as co-products
Auxiliary - kg and that have passed the end-of-waste state are included in
Other resources - kg module D. Such declared benefits can occur in stages A5 and
C4. The generated energy, such as heat and electricity from
Electricity consumption - kWh
waste incineration of packaging is assigned to module D. The
Other energy carriers - MJ
benefits are calculated using current average substitution
Material loss - kg processes. The heat is credited for with heat from natural gas.
The electricity is credited for with the specific country’s
Repair (B3)
electricity mix. This is also applied for materials that are
Name Value Unit landfilled as the benefits from electricity production from landfill
Information on the repair process - - gas recovery are included in module D.
Information on the inspection process - -
Repair cycle - Number/RSL Reuse, recovery and/or recycling potentials (D), relevant
Water consumption - m3 scenario information
Any declared benefits and loads from net flows leaving the
Auxiliary - kg
product system that have not been allocated as co-products
Other resources - kg
and that have passed the end-of-waste state are included in
Electricity consumption - kWh module D. Such declared benefits can occur in stages A5 and
Other energy carriers - MJ C4. The generated energy, such as heat and electricity from
Material loss - kg waste incineration of packaging is assigned to module D. The
benefits are calculated using current average substitution
Replacement (B4) / Refurbishment (B5) processes. The heat is credited for with heat from natural gas.
Name Value Unit The electricity is credited for with the specific country’s
electricity mix. This is also applied for materials that are
Replacement cycle - Number/RSL
landfilled as the benefits from electricity production from landfill
Electricity consumption - kWh
gas recovery are included in module D.
Litres of fuel - l/100km
Name Value Unit
Replacement of worn parts - kg
6 Environmental-Product Declaration - ROCKWOOL ROCKFON GmbH - Ceiling Tiles
LCA: Results
DESCRIPTION OF THE SYSTEM BOUNDARY (X = INCLUDED IN LCA; MND = MODULE NOT DECLARED; MNR = MODULE NOT
RELEVANT)
BENEFITS
AND LOADS
CONSTRUCTION
BEYOND
PRODUCT STAGE PROCESS USE STAGE END OF LIFE STAGE
THE SYSTEM
STAGE
BOUNDARIE
S
la ire ta m w a Ry lp p u s tro p s n a rT g n iru tc a fu n a M e h t m o rf tro p s n a rTe tis e h t o t e ta g y lb m e s s A e s U e c n a n e tn ia M ria p e R tn e m e c a lp e R tn e m h s ib ru fe R y g re n e la n o ita re p Oe s u re ta w la n o ita re p Oe s u n o itc u rts n o c -e Dn o itilo m e d tro p s n a rT g n is s e c o rp e ts a W la s o p s iD -e s u e R-y re v o c e R-g n ilc y c e Rla itn e to p
A1 A2 A3 A4 A5 B1 B2 B3 B4 B5 B6 B7 C1 C2 C3 C4 D
X X X X X MND X MNR MNR MNR X X X X X X X
RESULTS OF THE LCA - ENVIRONMENTAL IMPACT according to EN 15804+A1: 1 m² of Rockfon ceiling tile
Parameter Unit A1-A3 A4 A5 B2 B6 B7 C1 C2 C3 C4 D
GWP kg CO 2 eq 1.32E+00 2.21E-01 2.58E-01 0 0 0 0 4.79E-03 0 2.16E-02 -6.97E-02
kg CFC11
ODP 2.65E-09 3.66E-17 3.94E-10 0 0 0 0 7.93E-19 0 1.26E-16 -1.34E-14
eq
AP kg SO 2 eq 7.6E-03 1.87E-04 5.81E-04 0 0 0 0 4.38E-06 0 1.3E-04 -1.85E-04
EP kg PO 43 eq 1.17E-03 4.13E-05 1.02E-04 0 0 0 0 9.89E-07 0 1.47E-05 -1.8E-05
POCP kg Ethen eq 5.45E-04 7.02E-07 4.5E-05 0 0 0 0 -1.26E-07 0 9.96E-06 -1.79E-05
ADPE kg Sb eq 5.26E-07 1.71E-08 3.55E-08 0 0 0 0 3.7E-10 0 7.96E-09 -2.12E-08
ADPF MJ 1.56E+01 3.01E+00 1.4E+00 0 0 0 0 6.51E-02 0 3.03E-01 -1.42E+00
GWP = Global warming potential; ODP = Depletion potential of the stratospheric ozone layer; AP = Acidification potential of land and water; EP =
Eutrophication potential; POCP = Formation potential of tropospheric ozone photochemical oxidants; ADPE = Abiotic depletion potential for non-fossil
resources; ADPF = Abiotic depletion potential for fossil resources
RESULTS OF THE LCA - INDICATORS TO DESCRIBE RESOURCE USE according to EN 15804+A1: 1 m² of Rockfon ceiling tile
Parameter Unit A1-A3 A4 A5 B2 B6 B7 C1 C2 C3 C4 D
PERE MJ 3.4E+00 1.75E-01 2.05E+00 0 0 0 0 3.79E-03 0 3.97E-02 -2.06E-01
PERM MJ 2.2E+00 0 1.63E+00 0 0 0 0 0 0 0 0
PERT MJ 5.6E+00 1.75E-01 4.22E-01 0 0 0 0 3.79E-03 0 3.97E-02 -2.06E-01
PENRE MJ 1.53E+00 3.02E+00 1.58E+00 0 0 0 0 6.53E-02 0 3.14E-01 -1.53E+00
PENRM MJ 2.27E+00 0 -2.27E-02 0 0 0 0 0 0 0 0
PENRT MJ 1.76E+00 3.02E+00 1.56E+00 0 0 0 0 6.53E-02 0 3.14E-01 -1.53E+00
SM kg 0 0 0 0 0 0 0 0 0 0 0
RSF MJ 0 0 0 0 0 0 0 0 0 0 0
NRSF MJ 0 0 0 0 0 0 0 0 0 0 0
FW m3 6.19E-03 2.96E-04 8.11E-04 0 0 0 0 6.4E-06 0 7.9E-05 -4.23E-04
PERE = Use of renewable primary energy excluding renewable primary energy resources used as raw materials; PERM = Use of renewable primary
energy resources used as raw materials; PERT = Total use of renewable primary energy resources; PENRE = Use of non-renewable primary energy
excluding non-renewable primary energy resources used as raw materials; PENRM = Use of non-renewable primary energy resources used as raw
materials; PENRT = Total use of non-renewable primary energy resources; SM = Use of secondary material; RSF = Use of renewable secondary fuels;
NRSF = Use of non-renewable secondary fuels; FW = Use of net fresh water
RESULTS OF THE LCA – WASTE CATEGORIES AND OUTPUT FLOWS according to EN 15804+A1:
1 m² of Rockfon ceiling tile
Parameter Unit A1-A3 A4 A5 B2 B6 B7 C1 C2 C3 C4 D
HWD kg 3.59E-07 1.68E-07 3.77E-08 0 0 0 0 3.65E-09 0 5.35E-09 -1.7E-09
NHWD kg 1.2E-01 2.45E-04 1.17E-01 0 0 0 0 5.31E-06 0 1.46E+00 -8.99E-04
RWD kg 7.41E-04 4.09E-06 5.91E-05 0 0 0 0 8.86E-08 0 4.21E-06 -2.7E-05
CRU kg 0 0 0 0 0 0 0 0 0 0 0
MFR kg 0 0 3.42E-02 0 0 0 0 0 4.05E-02 0 0
MER kg 0 0 0 0 0 0 0 0 0 0 0
EEE MJ 0 0 1.53E-01 0 0 0 0 0 0 0 0
EET MJ 0 0 4.6E-01 0 0 0 0 0 0 0 0
HWD = Hazardous waste disposed; NHWD = Non-hazardous waste disposed; RWD = Radioactive waste disposed; CRU = Components for re-use;
MFR = Materials for recycling; MER = Materials for energy recovery; EEE = Exported electrical energy; EET = Exported thermal energy
References
7 Environmental-Product Declaration - ROCKWOOL ROCKFON GmbH - Ceiling Tiles
BBSR wool products: http://www.euceb.org/ [Accessed: July
2019].
GaBi ts
BBSR table "Service lives of components for life cycle Leinfelden - Echterdingen GaBi Software - System and
assessment Database for Life cycle Engineering. Thinkstep AG,
according to BNB", available via LBP, University of Stuttgart and PE. Program version
http://www.nachhaltigesbauen.de/baustoff-und- 8.0.1.257,database schema 8006 International, 2011.
gebaeudedaten/nutzungsdauern-von-bauteilen.html.
GaBi-Dokumentation
Thinkstep AG: GaBi 6 life cycle inventory data
documentation, 2018.
http://www.gabisoftware.com/support/gabi/gabi-6-
lcidocumentation [Accessed: July 2019].
ECHA PR/19/12
The Candidate List of substances of very high concern, ISO 15686 1-11
available via https://echa.europa.eu/nl/-/four-newsubstances- Series of standards for service life planning.
added-to-the-candidate-list, accessed October 2019
IBU PCR - Part A
Calculation rules for the Life Cycle Assessment and
EN ISO 717-1 Requirements on the Background Report, version 1.6,
EN ISO 717-1:2013, Acoustics — Rating of sound insulation in Institut Bauen und Umwelt e.V., www.bau-umwelt.com,
buildings and of building elements — Part 1: Airborne sound July 2019.
insulation
IBU 2017, PCR, Part B
PCR- Part B: Requirements on the EPD for mineral
insulating products, Institut Bauen und Umwelt e.V.,
EN ISO 10848-2 www.bau-umwelt.com, December 2018.
EN ISO 10848-2:2017, Acoustics — Laboratory and field
measurement of flanking transmission for airborne, impact and Regulation (EC) No 305/2011 CPR
building service equipment sound between adjoining rooms— Regulation (EC) No 305/2011 of the European
Part 2: Application to Type B elements when the junction has a Parliament and of the council of 9 March 2011 laying
small influence down harmonised conditions for the marketing of
construction products and repealing Council Directive
EN 13162 89/106/EEC. Available at: https://eurlex.
EN 13162:2008, Thermal insulation products for europa.eu/legalcontent/
buildings. Factory made mineral wool (MW) products. EN/TXT/?uri=celex%3A32011R0305.
Specification
Regulation (EC) No 1272/2008 - REACH
Regulation (EC) No 1272/2008 of the European
EN 13964 Parliament and of the council of 16 December 2008 on
EN 13964:2014, Suspended ceilings. Requirements and test classification, labeling and packaging of substances
methods and mixtures. Available at:
https://eurlex.europa.eu/legalcontent/EN/TXT/?uri=cele
x:32008R1272 [Accessed: July 2019].
EN 16516
EN 16516:2018, Construction products - Assessment of release The literature referred to in the Environmental Product
of dangerous substances - Determination of emissions into Declaration must be listed in full.Standards already fully quoted
indoor air in the EPD do not need to be listed here again.
The current version of PCR Part A and PCR Part B of the PCR
EUCEB document on which they are based must be referenced.
Website of European Certification Board for mineral
8 Environmental-Product Declaration - ROCKWOOL ROCKFON GmbH - Ceiling Tiles
Publisher
Institut Bauen und Umwelt e.V. +49 (0)30 3087748- 0
Hegelplatz 1 info@ibu-epd.com
10117 Berlin www.ibu-epd.com
Germany
Programme holder
Institut Bauen und Umwelt e.V. +49 (0)30 3087748- 0
Hegelplatz 1 info@ibu-epd.com
10117 Berlin www.ibu-epd.com
Germany
Author of the Life Cycle Assessment
ROCKWOOL ROCKFON GmbH +49 2043/408-0
Rockwool Straße 37-41 info@rockfon.de
D-4596 Gladbeck www.rockfon.de
Germany
Owner of the Declaration
ROCKWOOL ROCKFON GmbH +49 2043/408-0
Rockwool Straße 37-41 info@rockfon.de
D-4596 Gladbeck www.rockfon.de
Germany
9 Environmental-Product Declaration - ROCKWOOL ROCKFON GmbH - Ceiling Tiles
