ENVIRONMENTAL PRODUCT DECLARATION
as per ISO 14025 and EN 15804+A1
Owner of the Declaration Sto SE & Co. KGaA
Programme holder Institut Bauen und Umwelt e.V. (IBU)
Publisher Institut Bauen und Umwelt e.V. (IBU)
Declaration number EPD-IWM-STO-20210128-IBG1-DE
Issue date 07.07.2021
Valid to 06.07.2026
Mineral pre-made mortar: rendering mortar –
normal/finishing render
Sto SE & Co. KGaA
www.ibu-epd.com | https://epd-online.com
Umwelt Produktdeklaration Name des Herstellers – Name des Produkts
1. General Information
Sto SE & Co. KGaA Rendering mortar – normal/finishing
render
Programme holder Owner of the declaration
IBU – Institut Bauen und Umwelt e.V. Sto SE & Co. KGaA
Panoramastr. 1 Ehrenbachstraße 1
10178 Berlin D-79780 Stühlingen
Germany Germany
Declaration number Declared product / declared unit
EPD-IWM-STO-20210128-IBG1-DE 1 kg rendering mortar as a mineral pre-made mortar,
normal/finishing render product group with a dry bulk
density greater than 1300 kg/m³ and less than 1800
kg/m³.
Product names:
Sto Grundputz CP, Sto Putsbruk CP, Sto Putsbruk CP,
Sto Pudsmørtel CP, Sto Rappauslaasti CP, (DE, SE,
NO, DK, FI); Sto Grundputz BP, Sto Putsbruk BP, Sto
Putsbruk BP, Sto Pudsmørtel BP, Sto Rappauslaasti
BP, (DE, SE, NO, DK, FI); Sto Grundputz A, Sto
Putsbruk A, Sto Putsbruk A, Sto Pudsmørtel A, Sto
Rappauslaasti A, (DE, SE, NO, DK, FI); Sto Grundputz
B, Sto Putsbruk B, Sto Putsbruk B, Sto Pudsmørtel B,
Sto Rappauslaasti B, (DE, SE, NO, DK, FI); Sto
Grundputz C, Sto Putsbruk C, Sto Putsbruk C, Sto
Pudsmørtel C, Sto Rappauslaasti C, (DE, SE, NO, DK,
FI); Sto Kalkmörtel, Sto Kalkbruk, Sto Kalkbruk, Sto
Kalkmørtel, Sto Kalkkilaasti, (DE, SE, NO, DK, FI); Sto-
Hydraulischer Kalkmörtel Kh, Sto Hydrauliskt Kalkbruk
Kh, Sto Hydraulisk Kalkbruk Kh, Sto Hydraulisk
Kalkmørtel Kh, Sto Hydraulinen kalkkilaasti Kh, (DE,
SE, NO, DK, FI); Sto-Hydraulischer Kalkmörtel KKh,
Sto Hydrauliskt Kalkbruk KKh, Sto Hydraulisk Kalkbruk
KKh, Sto Hydraulisk Kalkmørtel KKh, Sto Hydraulinen
kalkkilaasti KKh, (DE, SE, NO, DK, FI);
This declaration is based on the product Scope:
category rules: This document is a model EPD. When calculating the
Mineral factory-made mortar, 11.2017 Life Cycle Assessment, the product selected to
(PCR checked and approved by the SVR) represent the group in question was the product with
the highest environmental impact in that group. This
EPD applies exclusively to rendering and plastering
Issue date
mortar – normal/finishing render or plaster as mineral
07.07.2021
pre-made mortars for association members; these can
be found on the association’s website. Any numerical
Valid to values – e.g. for constructional data or concentration
06.07.2026 specifications – are average values that are customary
in practice for this product group.
The owner of the declaration shall be liable for the
underlying information and evidence; the IBU shall not
be liable with respect to manufacturer information, life
cycle assessment data and evidences.
The EPD was created according to the specifications
of EN 15804+A1. In the following, the standard will be
simplified as EN 15804.
Verification
The standard EN 15804 serves as the core PCR
Independent verification of the declaration and data
according to ISO 14025:2010
Dipl. Ing. Hans Peters internally x externally
(chairman of Institut Bauen und Umwelt e.V.)
2 Environmental Product Declaration Sto SE & Co. KGaA – Mineral pre-made mortar: rendering and plastering mortar –
normal/finishing render or plaster
Dr. Alexander Röder Matthias Schulz
(Managing Director Institut Bauen und Umwelt e.V.)) (Independent verifier)
2. Product
2.1 Product description/Product definition %
Mineral pre-made mortars are mortars whose Thermal conductivity conductivity
components are mixed at the factory and not on the in accordance with DIN EN 1745 0,43 - 0,89 W/(mK)
construction site. They are divided into three different lambda10,dry,mat / P = 90 %
types – masonry mortar, rendering and plastering Sound absorption coefficient (as
- %
mortar, and screed material – depending on the type of required)
application. Water-vapour transmission rate in
15/35 -
Mineral rendering and plastering mortars are mixtures accordance with DIN EN 1015-19
of one or more mineral binders, aggregates, water, and Dry bulk density in accordance 1300 -
– if applicable – additions or admixtures for the with DIN EN 1015-10 1800 kg/m³
manufacture of renders or plasters. Rendering and Capillary absorption in accordance kg/(m²min
plastering mortars are applied to walls and ceilings in with DIN EN 1015-18 n/a ^0,5)
one or more layers as required. Alongside the
aesthetic design of the surface, they protect against
effects of the weather when used as external renders
Performance values of normal/finishing render or
and provide an even substrate for paint coats and
plaster according to the declaration of performance in
wallpaper when used as internal plasters. In the case
relation to its key characteristics in accordance with
of reinforced concrete ceilings and stairs,
DIN EN 998-1:2017-02, Specification for mortar for
renders/plasters also serve as fire protection; when
masonry - Part 1: Rendering and plastering mortar.
porous aggregates are added, they serve as thermal
Adhesive shear strength, bond strength, and flexural
protection. Depending on the technical data, the base
strength are not relevant.
materials and processing aids used, and the practical
application, rendering and plastering mortars are
2.4 Delivery status
divided into the following product groups:
Mineral rendering and plastering mortars –
normal/finishing render or plaster, normal/finishing
normal/finishing render or plaster are produced and
render, or plaster with special properties, lightweight
delivered as pre-made dry mortars. Pre-made dry
render, reinforcement fibre plaster, and insulating
mortar is a mortar made from raw materials that are
render with an especially high proportion of lightweight
placed into containers dry at the factory, delivered to
aggregates.
the construction site, and then mixed with the required
quantity of water to form ready-to-use mortar based on
Placing normal/finishing render or plaster on the
the manufacturer’s instructions and conditions.
market in the EU/EFTA (with the exception of
Delivered in sacks up to 35 kg per sack or in silos up to
Switzerland) is subject to Regulation (EU) No.
15 t per silo.
305/2011 (CPR). Normal/finishing render or plaster
requires a declaration of performance – taking into
2.5 Base materials/Ancillary materials
consideration DIN EN 998-1:2017-02, Specification for
mortar for masonry - Part 1: Rendering and plastering
Mineral building products such as mineral pre-made
mortar – and the CE marking.
mortars and rendering and plastering mortars mainly
The relevant national regulations apply with regard to
consist of abundant mineral raw materials. Scarcity of
usage.
resources is not an issue.
Name Value Unit
2.2 Application
Aggregate 55-70 M.-%
Rendering and plastering mortars produced in the
Fine aggregate 10-20 M.-%
factory for use as a base coat or finishing
Lightweight aggregate - M.-%
render/plaster on walls, ceilings, piers, and separating
Artificial lightweight aggregate - M.-%
walls of structures which comply with the applicable
Cement 7-20 M.-%
standards or on similar backgrounds (e.g. in the case
Hydrated lime [Ca(OH2] ≤ 17 M.-%
of existing buildings).
Normal render for the production of internal plaster and
The permissible fluctuation range of the constructional
external render without special properties.
data is enabled by the variety of proportions of base
materials. In each case, the composition of the
2.3 Technical Data
rendering and plastering mortars adds up to 100 m%.
Constructional data The following processing aids and admixtures can be
used as needed:
Name Value Unit
Compressive strength strength in  Synthetic dispersion: < 0.50 m%
≤ 15 N/mm2
accordance with DIN EN 1015-11  Water retention agent: < 0.30 m%
Thermal conductivity with DIN EN
0.39 - 0.82 W/(mK)  Air entraining admixture: < 0.03 m%
1745 lambda10,dry,mat / P = 50
 Thickening agent: < 0.03 m%  Conveyance of ingredients and substances
 Mineral pigments: < 0.20 m% being mixed into the mixer
 Hydrophobic agent: < 0.30 m%  Mixing
 Conveyance of finished products
Aggregate: Natural sands as natural raw materials,  Packaging
which contain natural minor and trace minerals along  Loading and shipping of the finished product
with the main minerals quartz (SiO2) or calcite
(CaCo3).
The raw materials – sand, binder, lightweight
Fine aggregate: Limestone dusts which arise as a
aggregates, processing aids, admixtures, and
result of the preparation of natural sand for the
additions (see base materials) – are stored at the
production of aggregates, as well as ultra-fine sands.
manufacturing plant in silos. From the silos, the raw
Lightweight aggregate: Natural or artificial mineral
materials are gravimetrically dosed and intensely
lightweight aggregates for reducing the dry bulk
mixed according to the respective formulation. The
density. Natural lightweight aggregates are
mixture is then packaged and shipped dry as pre-made
manufactured from natural raw materials via grinding
dry mortar in containers or silos.
(e.g. pumice or vermiculite). Artificial lightweight
aggregates are manufactured by processing, melting,
and swelling suitable natural raw materials (swelling
clay, perlite) or sorted recycled glass (expanded
glass).
Artificial lightweight aggregate: Organic, expanded
polystyrene (EPS) produced by foaming in spherical or
particle form (recycled) for reducing the dry bulk
density.
Cement: As per DIN EN 197-1; cement is used as a
binder and is mainly made from limestone marl or a
mixture of limestone and clay. The natural raw
materials are baked and then ground.
Hydrated lime: As per DIN EN 459; white hydrated
lime is used as a binder and is made by baking natural
limestone followed by slaking.
Synthetic dispersion: Polymer powder for improving
the adhesive bond, elasticity, mechanical properties,
etc. in thin-bed mortar.
Water retention agent: Cellulose ether, made from Graphic 1: Manufacturing process (green: input; blue:
cellulose, which prevents dehydration from occurring in unit process)
the fresh mortar too quickly.
Air entraining admixture: Surfactants for reducing 2.7 Environment and health during
the surface tension of water and producing entrained manufacturing
air. This reduces the bulk density of fresh mortar, The current state of the art includes the 100 % return
improves workability, and reduces the tendency of dry waste into production. In all places where dust
towards contraction and stress cracking. can arise during production in the factory, this waste is
Thickening agent: Cellulose or starch ether, made fed into a central filter system using the appropriate
from cellulose or crystal starch, improves the extraction systems, taking into account the
resistance to flow, and thus has a thickening effect, but occupational limit values. The very fine dust filtered out
does not have any water-retaining properties. in these systems is then fed back into the
Mineral pigments: Natural or synthetic powder-form manufacturing process. As part of the quality
colouring materials which are produced by mechanical management systems introduced, any off-specification
processing of the relevant mineral substances such as batches are detected immediately by the automated
chalk, clay, etc. process monitoring system and are fed into circulation
Hydrophobic agent: Water-soluble sodium oleate or via appropriate recovered-goods silos, i.e. they are fed
zinc stearate for reducing the capillary absorption of back into the production process in very small
the solid mortar. quantities. This procedure is also applied for product
residues which are transported back to the
Information about Substances of Very High Concern: manufacturing plant in small quantities in silos or
The product contains substances from the ECHA sacks.
candidate list (15.01.2019) above 0.1 % w/w: no. Process exhaust air is dedusted until the level is far
The product contains further CMR substances from below the statutory occupational limit values.
Category 1A or 1B which are not on the candidate list
above 0.1 % w/w in at least one part of the product: no. Noise:
Biocide products have been added to this building Noise level measurements have shown that all values
product or it has been treated with biocide products determined inside and outside the production facilities
(thus it is a treated product in the sense of the Biocide are well below the required specifications of the
Products Ordinance (EU) No. 528/2012): no. technical standards thanks to noise protection
measures being taken.
2.6 Manufacture
The graphic shows the manufacturing process. 2.8 Product processing/Installation
Mineral rendering and plastering mortars are made in Mineral rendering and plastering mortars are normally
mixing plants in the following steps: applied by machine. They are extracted from the silo
 Filling of the storage or weighing containers with a dry-materials conveying machine or from
4 Environmental Product Declaration Sto SE & Co. KGaA – Mineral pre-made mortar: rendering and plastering mortar –
normal/finishing render or plaster
individual containers and mixed with a mixing pump
before being conveyed and applied. Silo mixing pumps
can also be used. 2.13 Extraordinary effects
The rendering and plastering mortars are then levelled,
and textured if necessary, on site with suitable tools. Fire
The regulations of the employers’ liability insurance Fire protection class A1
associations and the respective safety data sheets of
the building products apply. The reaction to fire can be verified in the following
With the cement and lime binders in mineral pre-made ways in accordance with the regulations:
mortars, the fresh mortar mixed with water is strongly
alkaline. Prolonged contact can cause serious skin Option 1: Based on Commission Decision 94/611/EC,
damage owing to the alkalinity. Personal protective normal/finishing render or plaster is to be placed in fire
measures must therefore be taken (EU Health & protection class A1 “No contribution to fire” without
Safety Data Sheet) to avoid any contact with eyes or testing in accordance with DIN EN 13501-1 as the
skin. proportion of finely dispersed organic components is
No special measures are required for protection of the not greater than 1 %.
environment. Unchecked dust emissions must be Option 2: Because the proportion of finely dispersed
avoided. organic components is greater than 1 %, the fire
Mineral pre-made mortars must not enter the sewer protection class A1 is verified with a test as a matter of
system, surface water, or ground water. course.
2.9 Packaging Regardless of the product group, it has been shown in
Bagged cargo from a paper bag with a plastic insert, the “hot” measurement (structural analysis with the
sacks stored on wooden pallets, pallets wrapped in resistance of the masonry reduced under the influence
plastic film, silo-based goods stored in steel silos. of fire temperatures) that rendering and plastering
Possibilities of reuse for the packaging of bagged mortar made from mineral pre-made mortars has a
cargo – separation if necessary. Unsoiled polythene beneficial effect on the required minimum wall
films (correct sorting must be applied) and reusable thickness.
wooden pallets are taken back by the building material Depending on the product, additional labels will appear
dealer (reusable wooden pallets subject to on containers with the CE mark or declaration of
reimbursement as per the deposit system), returned to performance.
the mortar plants by the dealer, and fed back into the
production process. The films are forwarded to the film
manufacturers for recycling. Fire protection
Name Value
Building material class A1
2.10 Condition of use Burning droplets -
The specified products are rot-resistant and ageing- Smoke gas development -
resistant during normal use that conforms to the
intended purpose of the products described. Water
Rendering and plastering mortars made from mineral Mineral pre-made mortars as rendering and plastering
pre-made mortars must be protected from long-term mortars are structurally stable and are not subject to
weather effects, e.g. by properly connecting the facade changes in shape as a result of water exposure and
plinth (SAF). drying.
The cracking resistance of rendering and plastering
mortars made from mineral pre-made mortars can be Mechanical destruction
increased with cracking reinforcement in the tension- No specifications required.
stressed areas of the render DIN EN 13914-1, -2, DIN
18550-1, -2. 2.14 Re-use phase
The service life of masonry coated with
2.11 Environment and health during use normal/finishing render normally ends along with the
Due to the stable calcium silicate hydrate (CSH) service life of the simultaneously erected building.
adhesion and the firm structures achieved through Reuse and further use of masonry coated with render
curing on the substrate, emissions are rendered after demolition is not possible.
impossible. During normal use conforming to the Elements of building construction made from mineral
intended purpose of the products described, any rendering and plastering mortars can normally be
adverse health effects have been rendered impossible. stripped down easily. During demolition of a building,
No hazards for water, air, and soil are known for use these elements do not have to be treated as special
as per the intended application of the products. waste, but the sorting during demolition must be as
The natural ionising radiation of the rendering and exact as possible. Mineral rendering and plastering
plastering mortars made from mineral pre-made mortars can be recycled as building materials. They
mortars is extremely low and does not pose any are normally reused in structural and civil engineering
health-related risks. in the form of recycled aggregates.
2.12 Reference service life 2.15 Disposal
A reference service life (RSL) as per ISO 15686-1, -2, - Mortar is categorised as mineral construction waste.
7, and -8 is not declared. Provided they are used as 78.4 % of construction waste is recycled. German
intended and properly applied, the service life of Building Materials Association
rendering and plastering mortars made from mineral The suitability of hardened mineral rendering and
pre-made mortars on walls and ceilings has been plastering mortars for landfill as per landfill class I is
known to be 40 years or longer (BBSR).
5 Environmental Product Declaration Sto SE & Co. KGaA – Mineral pre-made mortar: rendering and plastering mortar –
normal/finishing render or plaster
ensured according to the Technical Instruction on 2.16 Further information
Municipal Waste (TASi). The EWC waste code Further information is available online at
according to the waste reuse directory is 170101. www.vdpm.info.
3. LCA: Calculation rules
3.1 Declared Unit All of the background records relevant to the
This declaration refers to the production of one assessment have been retrieved from the GaBi8
kilogram of typical rendering mortar of the database, with the exception of the pumice
normal/finishing render product group. Only dry (ROTOCELL) record.
mortars are taken into consideration.
3.6 Data quality
Specification of declared unit Representative products were used for this model EPD
– the product with the greatest environmental impact
Name Value Unit was declared to be representative of a group in order
Declared unit 1 kg to calculate the Life Cycle Assessment results.
1300 - Corresponding background records were available in
Gross density kg/m3
1800 the GaBi database for all relevant primary products
Spreading rate 0,70-0,85 l/kg used.
Conversion factor to 1 kg 1 - The requirements in terms of data quality and
background data correspond to the specifications of
The product which demonstrated the highest PCR Part A.
environmental impact of the normal/finishing render The technological background of the data collected
product group was selected from that group for reflects the physical reality for the declared product
calculating the Life Cycle Assessment. group.
The records are complete and fulfil the system
boundaries and criteria for the exclusion of inputs and
outputs.
The last audit of the data used was less than 8 years
ago.
3.2 System boundary
The lifecycle analysis of the products being examined
3.7 Period under review
encompasses the production of the mortar including
The period under review is one year of production
raw material extraction and the provision of energy
based on the year 2018. The reference area of the Life
sources up to the packaged, finished product (module
Cycle Assessments was limited to Germany. The
A1-A3), the application of the product including
result is that, besides production processes under
transportation to the construction site (module A4-A5),
these marginal conditions, the precursors also relevant
the usage phase (module B1), and disposal of the
for Germany, such as electricity and energy provision,
mortar (module C4). For silo-based goods, the
were used.
proportionate expenditure for transportation and
manufacturing of the silo is taken into account. Credit
3.8 Allocation
for packaging including energy recovery (module D) is
Specific information on the allocations within the
also incorporated into the Life Cycle Assessment.
background records can be found in the
documentation of the GaBi records. The material and
3.3 Estimates and assumptions
energy consumption for the declared product were
For the individual formulation components of the
allocated by the member companies of the VDPM. The
formulations, these were assessed according to
data made available consists of internal key figures
manufacturer specifications or literature in the event
which have not been published. A multi-input allocation
that no specific GaBi 8 processes were available.
is used as per a simple credit method with a credit for
power and thermal energy when burning packaging
3.4 Cut-off criteria
and production waste as well as the landfilling of
At the input side, all material flows that enter the
production waste. The credit from the disposal of
system and are greater than 1 % of their total mass or
packaging is credited in module D.
contribute more than 1 % to primary energy demand
are taken into consideration. The total amount of input
3.9 Comparability
flows not taken into consideration is maximum 5 % of
Basically, a comparison or an evaluation of EPD data
the energy and mass in use.
is only possible if all the data sets to be compared
The manufacturing of the machines, facilities, and
were created according to EN 15804 and the building
other infrastructure required for the production of the
context, respectively the product-specific
relevant products was not taken into consideration for
characteristics of performance, are taken into account.
the Life Cycle Assessments.
The GaBi 8 background database was used for
3.5 Background data
modelling purposes
The software system GaBi8 was used for modelling
the life cycle for the production of the mortar products.
4. LCA: Scenarios and additional technical information
6 Environmental Product Declaration Sto SE & Co. KGaA – Mineral pre-made mortar: rendering and plastering mortar –
normal/finishing render or plaster
The following technical information is necessary for the
declared modules or can be used for the development
of specific scenarios in the context of building
assessment if modules have not been declared (MND).
Transportation to the construction site (A4)
Name Value Unit
Litres of fuel 0.0062 l/100km
Transport distance 300 km
Capacity utilisation (including
50 - 85 %
empty runs)
Gross density of products 1300 -
kg/m3
transported 1800
Installation into the building (A5)
Name Value Unit
Auxiliary 0 kg
Water consumption 0.0003 m3
Other resources 0 kg
Electricity consumption 0.00045 kWh
Other energy carriers 0 MJ
Material loss 0 kg
Output substances following
0 kg
waste treatment on site
Dust in the air 0 kg
VOC in the air 0 kg
For use (B1) see Chapter 2.12 on use
In the use stage, the carbon dioxide absorbed by
means of carbonation is taken into consideration. The
carbon dioxide released during the neutralisation of
limestone (CaCO3) in the production of lime and
cement is reabsorbed when reacting with the lime and
cement binders, thus leading to an increase in
strength. In line with DIN EN 16757, the resulting
maximum theoretical carbon dioxide absorption for
fully carbonated rendering and plastering mortars and
the practical total maximum potential for carbon
dioxide absorption – taking into account the degree of
exposure of the surfaces – were calculated in the Life
Cycle Assessment of the pre-made mortar.
End of the life cycle (C1-C4)
Name Value Unit
Collected separately waste type 0 kg
Collected as mixed construction
0 kg
waste
Reuse 0 kg
Recycling 0 kg
Energy recovery 0 kg
Landfilling 1.04 kg
Reuse, recovery, and recycling potential (D);
relevant scenario specifications
Name Value Unit
Recycling silo (packaging) 100 %
Burning of wooden pallets
100 %
(packaging)
Burning of paper (packaging) 100 %
Burning of polythene film
100 %
(packaging)
7 Environmental Product Declaration Sto SE & Co. KGaA – Mineral pre-made mortar: rendering and plastering mortar –
normal/finishing render or plaster
5. LCA: Results
DESCRIPTION OF THE SYSTEM BOUNDARY (X = INCLUDED IN LCA; MND = MODULE NOT DECLARED;
MNR = MODULE NOT RELEVANT)
BENEFITS AND
CONSTRUCTI LOADS
PRODUCT STAGE ON PROCESS USE STAGE END OF LIFE STAGE BEYOND THE
STAGE SYSTEM
BOUNDARIES
8 Environmental Product Declaration Sto SE & Co. KGaA – Mineral pre-made mortar: rendering and plastering mortar –
normal/finishing render or plaster
lairetam
waR
ylppus tropsnarT
gnirutcafunaM
eht
morf
tropsnarT
etis
eht
ot
etag
ylbmessA esU
ecnanetniaM
riapeR
tnemecalpeR tnemhsibrufeR
ygrene
lanoitarepO esu
retaw
lanoitarepO esu
noitcurtsnoc-eD
noitilomed tropsnarT
gnissecorp
etsaW
lasopsiD -esueR -yrevoceR -gnilcyceR laitnetop
A1 A2 A3 A4 A5 B1 B2 B3 B4 B5 B6 B7 C1 C2 C3 C4 D
X X X X X X MND MNR MNR MNR MND MND MND MND MND X X
RESULTS OF THE LCA - ENVIRONMENTAL IMPACT according to EN 15804+A1: 1 kg Mineral pre-made
mortar: rendering and plastering mortar – normal/finishing render or plaster
Parameter Unit A1-A3 A4 A5 B1 C4 D
Global warming potential [kg CO2-Eq.] 2.08E-1 2.18E-2 4.17E-2 -1.08E-1 1.66E-2 -1.75E-2
Depletion potential of the stratospheric ozone layer [kg CFC11-Eq.] 4.97E-10 4.58E-16 5.71E-16 0.00E+0 3.69E-15 -1.27E-14
Acidification potential of land and water [kg SO2-Eq.] 2.78E-4 1.66E-5 5.46E-6 0.00E+0 9.80E-5 -1.91E-5
Eutrophication potential [kg (PO4)3--Eq.] 6.25E-5 3.74E-6 1.21E-6 0.00E+0 1.35E-5 -3.12E-6
Formation potential of tropospheric ozone photochemical
[kg ethene-Eq.] 2.79E-5 -2.35E-7 3.65E-7 0.00E+0 7.62E-6 -1.68E-6
oxidants
Abiotic depletion potential for non-fossil resources [kg Sb-Eq.] 9.43E-7 2.26E-9 7.30E-10 0.00E+0 6.37E-9 -4.04E-8
Abiotic depletion potential for fossil resources [MJ] 1.40E+0 2.92E-1 1.11E-2 0.00E+0 2.14E-1 -2.25E-1
RESULTS OF THE LCA - INDICATORS TO DESCRIBE RESOURCE USE according to EN 15804+A1: 1 kg
Mineral pre-made mortar: rendering and plastering mortar – normal/finishing render or plaster
Parameter Unit A1-A3 A4 A5 B1 C4 D
Renewable primary energy as energy carrier [MJ] 3.96E-1 1.97E-2 2.88E-1 0.00E+0 2.76E-2 -5.23E-2
Renewable primary energy resources as material utilization [MJ] 2.86E-1 0.00E+0 -2.86E-1 0.00E+0 0.00E+0 0.00E+0
Total use of renewable primary energy resources [MJ] 6.82E-1 1.97E-2 2.37E-3 0.00E+0 2.76E-2 -5.23E-2
Non-renewable primary energy as energy carrier [MJ] 1.50E+0 2.93E-1 4.93E-2 0.00E+0 2.22E-1 -2.53E-1
Non-renewable primary energy as material utilization [MJ] 3.70E-2 0.00E+0 -3.70E-2 0.00E+0 0.00E+0 0.00E+0
Total use of non-renewable primary energy resources [MJ] 1.54E+0 2.93E-1 1.23E-2 0.00E+0 2.22E-1 -2.53E-1
Use of secondary material [kg] 0.00E+0 0.00E+0 0.00E+0 0.00E+0 0.00E+0 0.00E+0
Use of renewable secondary fuels [MJ] 0.00E+0 0.00E+0 0.00E+0 0.00E+0 0.00E+0 0.00E+0
Use of non-renewable secondary fuels [MJ] 0.00E+0 0.00E+0 0.00E+0 0.00E+0 0.00E+0 0.00E+0
Use of net fresh water [m³] 4.44E-3 2.29E-5 4.02E-4 0.00E+0 4.23E-5 -3.33E-5
RESULTS OF THE LCA – WASTE CATEGORIES AND OUTPUT FLOWS according to EN 15804+A1:
1 kg Mineral pre-made mortar: rendering and plastering mortar – normal/finishing render or plaster
Parameter Unit A1-A3 A4 A5 B1 C4 D
Hazardous waste disposed [kg] 1.23E-8 1.88E-8 1.19E-11 0.00E+0 3.82E-9 -1.42E-10
Non-hazardous waste disposed [kg] 5.22E-3 2.18E-5 1.80E-4 0.00E+0 1.04E+0 -1.39E-4
Radioactive waste disposed [kg] 4.91E-5 3.54E-7 4.99E-7 0.00E+0 3.18E-6 -1.10E-5
Components for re-use [kg] 0.00E+0 0.00E+0 0.00E+0 0.00E+0 0.00E+0 0.00E+0
Materials for recycling [kg] 0.00E+0 0.00E+0 1.87E-4 0.00E+0 0.00E+0 0.00E+0
Materials for energy recovery [kg] 0.00E+0 0.00E+0 2.26E-2 0.00E+0 0.00E+0 0.00E+0
Exported electrical energy [MJ] 0.00E+0 0.00E+0 5.22E-2 0.00E+0 0.00E+0 0.00E+0
Exported thermal energy [MJ] 0.00E+0 0.00E+0 1.22E-1 0.00E+0 0.00E+0 0.00E+0
6. LCA: Interpretation
The LCA results are dominated by the life cycle hydrophobic agent, dispersion powder, and quartz
phases of raw material provision & transportation (A1 sand (together >80 % within A1). The manufacture of
& A2), manufacture (particularly the manufacture of the dispersion powder dominates the indicator ODP
packaging in A3), and landfill disposal (C4) in all (>95 %). The manufacture of the hydrophobic agent
impact categories. Taken together, approx. 60 – 90 % dominates the indicator ADPE (>95 %). Transportation
of the environmental impact comes from these life of the raw materials plays a secondary role (<10 % of
cycle phases. total A1-A2).
In total, raw materials used and their transportation The manufacture of the packaging contributes (with the
contribute (excluding ADPE and ODP) to the exception of GWP, ODP, ADPE, and PERT) approx.
environmental impact with a percentage of around 40 – 10 – 20 %. The use of wooden pallets and paper
70 % – primarily due to the use of limestone dust, contributes significantly to PERT (approx. 50 %
contribution) and leads to a low rate of carbon dioxide Landfill disposal at the end of the life cycle (C4)
absorption in A3 (<5 %). contributes (with the exception of ODP and ADPE)
approx. 0 – 20 % to the environmental impact.
Transportation of the products to the construction site
(A4) plays a secondary role (<10 %). In the use phase, around 30 % of the GWP caused is
reabsorbed by means of carbonation (= carbon dioxide
absorption).
7. Requisite evidence
7.1 Leaching: All specified products remained below the
All specified products in this LCA comply with all recommended limiting value.
emissions scenarios for a scenario involving the
building elements that are subject to moisture. 7.3 Radioactivity:
Measuring location: Fraunhofer Institute for Building
7.2 VOC emissions: Physics (IBP), Holzkirchen Branch, D-83626 Valley
Measuring location: Fraunhofer Institute for Building Measuring procedure: Test of content for the
Physics (IBP), Holzkirchen Branch, D-83626 Valley radioactive nuclides radium-226, thorium-232, and
Measuring procedure: Determination of volatile potassium-40 by measuring the activity concentrations
organic compounds from building products and fixtures CNuclide through alpha spectrometry (delayed
in accordance with DIN EN ISO 16000-9 and -11 in a coincidence method via LSC) or gamma spectrometry
0.2 m3 test chamber (t0 = 7 days) and evaluation as Test report: Inspection report from 12 December 2006
per the schema of the Committee for Health-related on the radioactivity of building products
Evaluation of Building Products (AgBB). Measurement Result: The activity concentration indices (I) calculated
of different products intended for both interior use and from the measured activity concentrations CNuclide
outdoors. were below the recommended limiting value of I = 2 for
Test report: Results log 005/2008/281 from 20 March all specified products. Moreover, at no point was the
2008 recommended limiting value I = 0.5 either reached or
Results: exceeded for building products used in large
quantities. Where I correlated with the dose criterion in
accordance with the Radiation Protection 112
guidelines from the European Commission, all
specified products remained below the recommended
limiting value of the annual radiation dose of 0.3
mSv/a.
8. References
PCR guidelines on building-related products and Core rules for the product category of construction
services, Part A: Calculation rules for the Life Cycle products.
Assessment and requirements on the project report,
Institut Bauen und Umwelt e. V., Version 1.7, 2018-03 GaBi 8
GaBi 8.7 dataset documentation for the software-
PCR guidelines on building-related products and system and databases, LBP, University of Stuttgart
services, Part B: Requirements on the EPD for and thinkstep, Leinfelden-Echterdingen, 2018
mineral pre-made mortars, Institut Bauen und Umwelt (http://documentation.gabi-software.com/)
e. V., Version 1.6, 2017-11
IBU 2016 DIN 4108-4
IBU (2016): General EPD programme instructions from DIN 4108-4:2017-03, Thermal insulation and energy
the economy in buildings - Part 4: Hygrothermal design
Institut Bauen und Umwelt e.V. (IBU). Version 1.1, values
Institut Bauen und Umwelt e.V., Berlin.
DIN 18550-1
ISO 14025 DIN 18550-1:2018-01, Design, preparation and
DIN EN ISO 14025:201110, application of external rendering and internal
Environmental labels and declarations - type III plastering - Part 1: Supplementary provisions for
environmental declarations - principles and DIN EN 13914-1:2016-09 for external rendering
procedures.
DIN 18550-2
EN 15804 DIN 18550-2:2018-01, Design, preparation and
EN 15804:201204+A1 2013, Sustainability of application of external rendering and internal
construction works - Environmental product plastering - Part 2: Supplementary provisions for
declarations - DIN EN 13914-2:2016-09 for internal plastering
9 Environmental Product Declaration Sto SE & Co. KGaA – Mineral pre-made mortar: rendering and plastering mortar –
normal/finishing render or plaster
DIN EN 13914-2 Corrigendum 1
DIN EN 197-1 DIN EN 13914-2 Corrigendum 1:2017-05, Design,
DIN EN 197-1:2011-11, Cement - Part 1: Composition, preparation and application of external rendering and
specifications, and conformity criteria for common internal plastering - Part 2: Internal plastering;
cements Corrigendum to DIN EN 13914-2:2016-09
DIN EN 450-1 DIN EN 16757
DIN EN 450-1:2012-10, Fly ash for concrete - Part 1: DIN EN 16757:2017-10, Sustainability of construction
Definition, specifications, and conformity criteria works - Environmental product declarations - Product
Category Rules for concrete and concrete elements
DIN EN 459-1
DIN EN 459-1:2015-07, Building lime - Part 1: DIN EN ISO 14040
Definitions, specifications, and conformity criteria DIN EN ISO 14040:2009-11, Environmental
management - Life cycle assessment - Principles and
DIN EN 998-1 framework (ISO 14040:2006)
DIN EN 998-1:2017-02, Specification for mortar for
masonry - Part 1: Rendering and plastering mortar DIN EN ISO 14044
DIN EN ISO 14044:2018-05, Environmental
DIN EN 1015-10 management - Life cycle assessment - Requirements
DIN EN 1015-10:2007-05, Methods of test for mortar and guidelines (ISO 14044:2006 + Amd 1:2017)
for masonry - Part 10: Determination of dry bulk
density of hardened mortar DIN EN ISO 16000-9
DIN EN ISO 16000-9:2008-04, Indoor air - Part 9:
DIN EN 1015-11 Determination of the emission of volatile organic
DIN EN 1015-11:2007-05, Methods of test for mortar compounds from building products and furnishing -
for masonry - Part 11: Determination of flexural and Emission test chamber method
compressive strength of hardened mortar
DIN EN ISO 16000-11
DIN EN 1015-18 DIN EN ISO 16000-11:2006-06, Indoor air - Part 11:
DIN EN 1015-18:2003-03, Methods of test for mortar Determination of the emission of volatile organic
for masonry - Part 18: Determination of water compounds from building products and furnishing -
absorption coefficient due to capillary action of Sampling, storage of samples and preparation of test
hardened mortar specimens
DIN EN 1015-19 EC safety data sheet
DIN EN 1015-19:2005-01, Methods of test for mortar Available on the website of the relevant VDPM
for masonry - Part 19: Determination of water vapour member company.
permeability of hardened rendering and plastering
mortars ISO 15686-1
ISO 15686-1:2011-05, Buildings and constructed
DIN EN 1052-3 assets – Service life planning – Part 1: General
DIN EN 1052-3:2007-06, Methods of test for masonry - principles and framework
Part 3: Determination of initial shear strength
ISO 15686-2
DIN EN 1745 ISO 15686-2:2012-05, Buildings and constructed
DIN EN 1745:2012-07 Masonry and masonry products assets – Service life planning – Part 2: Service life
- Methods for determining thermal properties prediction procedures
DIN EN 12664 ISO 15686-7
DIN EN 12664: 2001-05, Thermal performance of ISO 15686-7:2017-04, Buildings and constructed
building materials and products - Determination of assets - Service life planning - Part 7: Performance
thermal resistance by means of guarded hot plate and evaluation for feedback of service life data from
heat flow meter methods - Dry and moist products with practice
medium and low thermal resistance
ISO 15686-8
DIN EN 13501-1 ISO 15686-8:2008-06, Buildings and constructed
DIN EN 13501-1:2010-01, Fire classification of assets - Service-life planning - Part 8: Reference
construction products and building elements - Part 1: service life and service-life estimation
Classification using data from reaction to fire tests
AgBB
DIN EN 13914-1 Committee for Health-related Evaluation of Building
DIN EN 13914-1:2016-09, Design, preparation and Products (AgBB): Procedure for the health-related
application of external rendering and internal plastering evaluation of volatile organic compound (VOC)
- Part 1: External rendering emissions from building products
DIN EN 13914-2 AVV
DIN EN 13914-2:2016-09, Design, preparation and Waste Catalogue Ordinance dated 10 December 2001
application of external rendering and internal plastering (Federal Law Gazette I p. 3379), last amended by
- Part 2: Internal plastering Article 2 of the Regulation of 17 July 2017 (Federal
Law Gazette I. p. 2644)
10 Environmental Product Declaration Sto SE & Co. KGaA – Mineral pre-made mortar: rendering and plastering mortar –
normal/finishing render or plaster
BBSR mixed dry render), January 2000 edition (unpublished)
BBSR - Federal Office for Building and Regional
Planning: Nutzungsdauern von Bauteilen für Commission Decision 94/611/EC
Lebenszyklusanalysen nach Bewertungssystem Commission Decision of 9 September 1994
Nachhaltiges Bauen (BNB) (Service lives of building implementing Article 20 of Directive 89/106/EEC on
elements for Life Cycle Assessments conducted construction products (94/611/EC)
according to the BNB Sustainable Building assessment
system), dated 24 February 2017 Life Cycle Assessment
Comparative Life Cycle Assessment: Masonry with
German Building Materials Association mineral mortar and masonry with PU foam bonding in
Bundesverband Baustoffe – Steine und Erden accordance with ISO 14040 and ISO 14044; carried
(German Building Materials Association) (Ed.): out on behalf of the VDPM (formerly IWM); Fraunhofer
Mineralische Bauabfälle – Monitoring 2010 (Mineral Institute for Building Physics IBP, Stuttgart/Holzkirchen
construction waste – monitoring 2010); Berlin, 2013 2008
DepV (2009) Radiation Protection 112
Ordinance on Landfills and Long-Term Storage European Commission: Radiation Protection 112
Facilities – Landfill Ordinance of 27 April 2009 (Federal “Radiological protection principles concerning the
Law Gazette I p. 900); last modified by Article 2 of the natural radioactivity of building materials”,
Regulation of 27 September 2017 (Federal Law Luxembourg: Publications Office of the European
Gazette I p. 3465). Union, 2000
ECHA candidate list SAF
European Chemicals Agency (ECHA): List of SAF – Fachverband der Stuckateure für Ausbau und
Substances of Very High Concern (published in Fassade Baden-Württemberg e.V. (Association of
accordance with Article 59 Para. 10 of the REACH Plasterers for Finishing and Facade) (Ed.): “Facade
Regulation) base render / outside facilities” guidelines, 3rd edition
2013
EWC waste code
Ordinance regarding the introduction of the European TASi
Waste Catalogue (EWC Ordinance) from 13 Technical Guidelines for the Recovery, Treatment and
September 1996: six-figure designation of types of Other Forms of Management of Domestic Waste (Third
waste, provided movable objects are waste according General Administrative Regulation for the Waste Act)
to Art. 3 Para. 1 of the Closed Substance Cycle and from 14 May 1993 (Federal Gazette No. 99a of 29 May
Waste Management Act 1993)
Industrieverband Werktrockenmörtel e.V. (WTM)
Internal study “Ökologische Aspekte von
Werktrockenmörtel” (Ecological aspects of ready
11 Environmental Product Declaration Sto SE & Co. KGaA – Mineral pre-made mortar: rendering and plastering mortar –
normal/finishing render or plaster
Publisher
Institut Bauen und Umwelt e.V. Tel +49 (0)30 3087748- 0
Panoramastr. 1 Fax +49 (0)30 3087748- 29
10178 Berlin Mail info@ibu-epd.com
Germany Web www.ibu-epd.com
Programme holder
Institut Bauen und Umwelt e.V. Tel +49 (0)30 - 3087748- 0
Panoramastr 1 Fax +49 (0)30 – 3087748 - 29
10178 Berlin Mail info@ibu-epd.com
Germany Web www.ibu-epd.com
Author of the Life Cycle
Assessment Tel +49 711 341817-0
thinkstep AG Fax +49 711 341817-25
Hauptstraße 111- 113 Mail info@thinkstep.com
70771 Leinfelden-Echterdingen Web http://www.thinkstep.com
Germany
Owner of the Declaration
Sto SE & Co. KGaA Tel +49 7744 57-1010
Ehrenbachstr. 1 Fax +49 7744 57-2010
79780 Stühlingen Mail infoservice@sto.com
Germany Web www.sto.com
Verband für Dämmsysteme, Putz Tel +49 (0)30 403670750
und Mörtel e.V. Fax +49 (0)30 403670759
Reinhardtstraße 14 Mail info@vdpm.info
10117 Berlin Web www.vdpm.info
Germany
