ENVIRONMENTAL PRODUCT DECLARATION
as per ISO 14025 and EN 15804+A2
Owner of the Declaration Shaw Contract (Shaw Europe Ltd.)
Publisher Institut Bauen und Umwelt e.V. (IBU)
Programme holder Institut Bauen und Umwelt e.V. (IBU)
Declaration number EPD-SHA-20230440-CBA1-EN
Issue date 06.11.2023
Valid to 05.11.2028
EcoWorx® Carpet Tile (US Made UK Market) with EcoSolution Q®,
Solution Q®, or Solution Q Extreme® Face Fibre
Shaw Contract (Shaw Europe Ltd.)
www.ibu-epd.com | https://epd-online.com
General Information
Shaw Contract (Shaw Europe Ltd.) EcoWorx® Carpet Tile (US Made UK Market) with
EcoSolution Q®, Solution Q®, or Solution Q
Extreme® Face Fibre
Programme holder Owner of the declaration
IBU – Institut Bauen und Umwelt e.V. Shaw Contract (Shaw Europe Ltd.)
Hegelplatz 1 Blackaddie Road *
10117 Berlin DG46DB Sanquhar
Germany United Kingdom
Declaration number Declared product / declared unit
EPD-SHA-20230440-CBA1-EN 1 m2 of installed EcoWorx® Carpet Tile
This declaration is based on the product category rules: Scope:
Floor coverings, 01.08.2021 A Life Cycle Assessment (LCA) was conducted based upon production
(PCR checked and approved by the SVR) data collected from Shaw Contract (Shaw Europe, Ltd.), Plant SQ
manufacturing facility (Blackaddie Road, Sanquhar, DG46DB), located in
Scotland, UK. Production data was collected for EcoWorx® Carpet Tile (US
Issue date Made UK Market) with EcoSolution Q®, Solution Q®, or Solution Q
06.11.2023 Extreme® Face Fibre, for the period of one year, from January to
December 2021.
Valid to This EPD is cradle-to-gate with options in scope with additional modules
A4, A5, B1 and B2. The EPD is created in accordance to the specifications
05.11.2028
of EN 15804+A2.
The EPD was generated with the help of Envision LCA Tool, version 1. The
tool has not been manipulated in calculating impact results. The current
version of the tool is maintained, saved, and stored for 10 years to be used
for revision and re-traceability purposes.
The owner of the declaration shall be liable for the underlying information
and evidence; the IBU shall not be liable with respect to manufacturer
information, life cycle assessment data and evidences.
The EPD was created according to the specifications of EN 15804+A2. In
the following, the standard will be simplified as EN 15804.
Dipl.-Ing. Hans Peters
(Chairman of Institut Bauen und Umwelt e.V.) Verification
The standard EN 15804 serves as the core PCR
Independent verification of the declaration and data according to ISO
14025:2011
internally X externally
Florian Pronold Mrs Kim Allbury,
(Managing Director Institut Bauen und Umwelt e.V.) (Independent verifier)
Environmental Product Declaration - Shaw Contract (Shaw Europe Ltd.) - EcoWorx® Carpet Tile (US Made UK Market) with EcoSolution Q®, Solution Q®, or Solution Q
1 Extreme® Face Fibre
Product
Name Value Unit
Product description/Product definition
Product thickness 6.53 mm
This EPD applies to carpet tile with EcoWorx® backing system
Grammage 3087 g/m2
together with EcoSolution Q®, Solution Q®, or Solution Q
Extreme® Nylon face fibre. EcoWorx® is a commercial carpet Product Form Carpet Tile -
tile, for use as a floor covering in accordance with Yarn type - Solution-dyed 1% Post-industrial
-
manufacturer's guidelines. Nylon 6 Recycled Content
Total thickness 6.53 mm
The carpet tile consists of Shaw's unique face fibre, Nylon 6, Total carpet weight 3087 g/m2
manufactured with 1% recycled material on EcoWorx® backing
Surface pile thickness 2.74 mm
system, a polyolefin-based compound which also includes
Surface pile weight - Nominal
recycled materials and a fibreglass secondary reinforcement 664.5 g/m2
Pile Mass
layer.
Length and width of squared
250 - 1000 mm
The EcoSolution Q®, Solution Q®, or Solution Q Extreme® face elements
fibre is tufted into a primary backing sheet containing recycled Other technical data parameters listed in IBU PCR Part B are
content. Latex is added to anchor the fibre and the not relevant and, therefore, have not been declared.
EcoWorx® backing system is then applied.
Performance data of the product in accordance with the
EcoWorx® is suitable for use in all commercial settings. It has a declaration of performance with respect to its essential
life span of 15 years, and it comes with a 15-year warranty characteristics according to 14041:2004A/C:2006.
(subject only to installation and maintenance being carried out
Base materials/Ancillary materials
in line with manufacturer's guidelines).
EcoWorx® Carpet Tile (US Made UK Market) with EcoSolution
This product meets both internal and external performance Q®, Solution Q®, or Solution Q Extreme® Face Fibre is
standards including those established in the EU under EN 1307 comprised of the following raw materials:
and EN 10874 for a product suitable for heavy and general
• 40-45% Calcium Carbonate, containing Recycled
commercial installations.
Content
For the placing on the market of the product in the European
• 9-12% Polyethylene
Union/European Free Trade Association (EU/EFTA) (with the
• 20-24% Solution-dyed Nylon 6 Face Fibre, containing
exception of Switzerland) Regulation (EU) No. 305/2011 (CPR)
1% Post-industrial Recycled Content
applies. The product needs a declaration of performance taking
• 3-5% Polyester Primary & Secondary Backing
into consideration EN 14041:2004A/C:2006, and the CE-
• 1-3% Fibreglass Reinforcement
marking.
• 0-1% Topical layer
• 10-27% Proprietary Raw Materials
For the application and use, the respective national provisions
The product is packaged in cardboard boxes, wrapped in
apply.
plastic, and stacked on wooden pallets for distribution.
Application
The product fits into the defined scope and all raw material
EcoWorx® Carpet Tile (US Made UK Market) with EcoSolution
inputs, with no exceptions, are captured by the Envision LCA
Q®, Solution Q®, or Solution Q Extreme® Face Fibre is suitable
Tool, version 1.
for use as a floor covering in heavy and general commercial
installations.
This product contains substances listed in the candidate list
(date: 17.01.2023) exceeding 0.1 percentage by mass: no
Technical Data
The technical specifications of the product are listed on the
This product contains other CMR substances in categories 1A
product's specification sheet, found at www.shawcontract.com.
or 1B which are not on the candidate list, exceeding 0.1
This product meets the requirements of the harmonized
percentage by mass: no
European Norm (hEN): EN14041:2004A/C:2006. Declarations
of performance related to fire, electrostatic, formaldehyde
Biocide products were added to this construction product or it
emissions, and slip resistance can be found on the product's
has been treated with biocide products (this then concerns a
specification sheet.
treated product as defined by the (EU) Ordinance on Biocide
Constructional data Products No. 528/2012): no
Reference service life
When properly installed as a commercial floor covering,
EcoWorx® Carpet Tile (US Made UK Market) with EcoSolution
Q®, Solution Q®, or Solution Q Extreme® face fibre has a
reference service life of 15 years. This carpet tile product
comes with a 15-year warranty, subject only to installation and
maintenance being carried out in accordance with the
manufacturer's guidelines.
LCA: Calculation rules
Environmental Product Declaration - Shaw Contract (Shaw Europe Ltd.) - EcoWorx® Carpet Tile (US Made UK Market) with EcoSolution Q®, Solution Q®, or Solution Q
2 Extreme® Face Fibre
• Module B4 - Replacement (module not relevant).
Declared Unit • Module B5 - Refurbishment (module not relevant).
The declaration refers to the declared unit of 1 m² of installed • Module B6 - Operational Energy Use (module not
carpet tile. relevant).
Declared unit • Module B7 - Operational Water Use (module not
relevant).
Name Value Unit
End of Life Stage:
Declared unit 1 m2 Three scenarios have been evaluated:
Grammage 3.087 kg/m2 Scenario 1: the EcoWorx® (US Made UK Market) carpet is
Layer thickness 0.00653 m 100% disposed of in a landfill.
Scenario 2: the EcoWorx® (US Made UK Market) carpet is
System boundary 100% incinerated.
The type of EPD is Cradle-to-Gate with options modules C1– Scenario 3: 40% of EcoWorx® (US Made UK Market) carpets
C4, module D, and additional modules. The additional modules are incinerated and the remaining 60% are landfilled. This
are A4, A5, B1 and B2. assumption is based on the carpet disposal rates in Europe
mentioned in the study conducted by Deutsche Umwelthilfe in
The modules considered in the life cycle assessment and 2017 (Umwelthilfe, 2017) and the European Commission in
environmental product declaration, based on the product's 2013 (Commission, 2013).
entire life cycle, are described as follows: • Module C1 - The carpet is de-constructed manually and
no additional environmental impact is caused.
Production Stage: • Module C2 - Transport of the carpet waste to a landfill or
• Module A1 - Provision of Raw Materials. to the municipal waste incineration plant.
• Module A2 - Transport of Raw Materials. • Module C3 - Impacts from thermal treatment disposal
• Module A3 - Manufacturing. (C3/2 and C3/3).
Construction/Installation Stage: • Module C4 - Impacts from landfill disposal (C4/1 and
C4/3).
• Module A4 - Transportation by truck of the product to the
Module D includes benefits from energy recovery via treatment
construction site in Europe.
of packaging materials and incineration of carpets at their end
• Module A5 - Installation of the carpet, treatment of
of life (D/1, D/2 and D/3), as well as the burdens of balancing
cutting waste (landfill) and packaging waste (landfill,
the secondary material content in modules A1 and A3 via the
recycling, and incineration). The production of the
net-scrap approach.
amount of carpet that occurs as installation waste is
also included along with its transport to the place of Geographic Representativeness
installation. Biogenic carbon that is stored in the wooden Land or region, in which the declared product system is
pallets and cardboard (packaging) is released as carbon manufactured, used or handled at the end of the product´s
dioxide emissions into the air at the end of life in module lifespan: Europe
A5.
Use Stage:
Comparability
• Module B1 - Indoor emissions of volatile organic
Basically, a comparison or an evaluation of EPD data is only
compounds (VOCs) during the first few months after
possible if all the data sets to be compared were created
installation.
according to EN 15804 and the building context, respectively
• Module B2 - Carpet cleaning per year, including
the product-specific characteristics of performance, are taken
vacuuming (electricity consumption) and hot water
into account. The background database used for the creation of
cleaning (electricity and water consumption, as well as
the EPD: GaBi ts software, CUP 2022.2.
waste water treatment).
• Module B3 - Repair (module not relevant).
LCA: Scenarios and additional technical information
Installation in the building (A5)
Characteristic product properties of biogenic carbon
Biogenic carbon is only present in packaging (wooden pallets The installation of EcoWorx® (US Made UK Market) is is done
and cardboards). Assumed water content in wooden pallet manually and no energy is required. A Pressure-Sensitive
(packaging): 18%. adhesive is required for the installation of EcoWorx® (US Made
UK Market) carpet tile and should be used in accordance with
Information on describing the Biogenic Carbon Content at
the manufacturer's guidelines. Installation losses have been
factory gate
accounted for in module A5. Product losses are considered as
Name ValueUnit 5%.
Biogenic carbon content in accompanying kg
0.14
packaging C The packaging material treatment and disposal are also
considered in module A5 (landfill, recycling, and incineration)
and the resulting benefits from energy generation are included
The following technical scenario information is required for the
in module D. The quantity of wooden pallets used is 0.133 kg
declared modules and optional for non-declared modules.
per m². Wooden pallets are assumed to be re-used 20 times
Transport to the construction site (A4) before being disposed of. Hence, the quantity of pallet disposed
Name Value Unit is 0.007 kg. The quantity of cardboard packaging is 0.21 kg/m²
Transport distance (truck) 687 km and the quantity of plastic packaging is 0.0103 kg/m². Total
amount of packaging disposed at installation is 0.227 kg.
Capacity utilisation (including empty runs) 55 %
Packaging disposal rates (Source: Eurostat, Recovery and
Environmental Product Declaration - Shaw Contract (Shaw Europe Ltd.) - EcoWorx® Carpet Tile (US Made UK Market) with EcoSolution Q®, Solution Q®, or Solution Q
3 Extreme® Face Fibre
recycling rates for packaging).
End of Life (C1-C4)
• Paper - 82.8% recycled; 9.4% landfilled; and 7.8% C1 - The product dismantling from the building is done
incinerated manually without energy burden.
• Plastic - 40.3% recycled; 28.7% landfilled; and 31.0% C2 - Transportation of the product to the end of life is assumed
incinerated to be 161 km (100 miles).
• Wood pallets - 39.8% recycled; 34.5% landfilled; and C3/2 - The EcoWorx® (US Made UK Market) carpet is 100%
25.7% incinerated combusted in an incineration plant with energy recovery
Name ValueUnit (R>0.6).
Auxiliary 0.23 kg C3/3 - It is assumed that 40% of EcoWorx® (US Made UK
Material loss 0.154 kg Market) carpets are incinerated and the remaining 60% are
landfilled.
Output substances following waste treatment on
site (packaging materials) 0.227 kg C4/1 - The EcoWorx® (US Made UK Market) carpet is 100%
disposed of in landfill.
Use (B1) see cap. 2.12 use C4/3 - It is assumed that 40% of EcoWorx® (US Made UK
Name Value Unit Market) carpets are incinerated and the remaining 60% are
landfilled.
Emissions to air (TVOC) after 50 days - Indoor Air
900 mg/m²
Comfort Gold® Name ValueUnit
Collected as mixed construction waste 3.087 kg
Emission testing was conducted in accordance to Eurofins
Indoor Air Comfort Gold® certification. After 28 days, the Landfilling (Scenario 1 - C3/1, C4/1 and D/1) 3.087 kg
specific concentration of TVOCs was <100 ug/m3, as required Incineration (Scenario 2 - C3/2, C4/2, and D/2) 3.087 kg
by the certification standard. Landfilling (60%) and Incineration (40%) (Scenario
3.087 kg
3 - C3/3, C4/3 and D/3)
Maintenance (B2)
For the maintenance of EcoWorx® (US Made UK Market) Reuse, recovery and/or recycling potentials (D), relevant
Carpet Tile, 2 hot water extraction cleanings (water and scenario information
electricity consumption) per year as well as 52 vacuum For the thermal and electrical energy generated in Module A5
cleanings (electricity consumption) per year are recommended. due to thermal treatment of packaging, avoided burdens have
The Reference Service Life of the product is 15 years. The been calculated by the inversion of electricity grid mix and
results in the EPD declare a maintenance for the period of 1 thermal energy from natural gas, using European datasets.
year. Module D also includes the environmental burdens linked to the
supply to secondary materials (nylon and calcium carbonate)
Name Value Unit
used in the carpet production.
Water consumption (1 year) 0.0009 m3
Electricity consumption (1 year) 0.772 kWh
Reference service life
Name ValueUnit
Reference service life (according to ISO 15686-1, -
15 a
2, -7 and -8)
Life Span according to the manufacturer 15 a
Environmental Product Declaration - Shaw Contract (Shaw Europe Ltd.) - EcoWorx® Carpet Tile (US Made UK Market) with EcoSolution Q®, Solution Q®, or Solution Q
4 Extreme® Face Fibre
LCA: Results
The B2 module declares the maintenance (cleaning) per one year. The user of the EPD will be able to scale the results for its entire
useful life by multiplying the impact by the RSL.
The LCA results presented below applies to 100% landfilled end of life scenario.
DESCRIPTION OF THE SYSTEM BOUNDARY (X = INCLUDED IN LCA; MND = MODULE OR INDICATOR NOT DECLARED; MNR
= MODULE NOT RELEVANT)
Benefits and
Construction loads beyond
Product stage Use stage End of life stage
process stage the system
boundaries
la ire ta m w a Ry lp p u s tro p s n a rT g n iru tc a fu n a M e h t m o rf tro p s n a rTe tis e h t o t e ta g y lb m e s s A e s U e c n a n e tn ia M ria p e R tn e m e c a lp e R tn e m h s ib ru fe R y g re n e la n o ita re p Oe s u re ta w la n o ita re p Oe s u n o itc u rts n o c -e Dn o itilo m e d tro p s n a rT g n is s e c o rp e ts a W la s o p s iD -e s u e R-y re v o c e R-g n ilc y c e Rla itn e to p
A1 A2 A3 A4 A5 B1 B2 B3 B4 B5 B6 B7 C1 C2 C3 C4 D
X X X X X X X MNR MNR MNR MND MND X X X X X
RESULTS OF THE LCA - ENVIRONMENTAL IMPACT according to EN 15804+A2: 1 m² EcoWorx® Carpet (US Made UK Market)
Parameter Unit A1-A3 A4 A5 B1 B2 C1 C2 C3 C4 D
GWP-total kg CO 2 eq 8.67E+00 1.98E-01 5.57E-01 2.54E-04 2.89E-01 0 4.18E-02 0 2.17E-01 4.38E-02
GWP-fossil kg CO 2 eq 9.08E+00 1.97E-01 5.65E-01 2.54E-04 2.86E-01 0 4.16E-02 0 2.19E-01 3.97E-02
GWP-
biogenic kg CO 2 eq -4.14E-01 -2.72E-04 -8.14E-03 0 3.05E-03 0 -5.75E-05 0 -2.33E-03 4.15E-03
GWP-luluc kg CO 2 eq 6.12E-04 1.1E-03 1.25E-04 0 6.06E-05 0 2.32E-04 0 1.07E-04 1.94E-05
ODP kg CFC11 eq 8.26E-09 1.18E-14 4.35E-10 0 4.19E-12 0 2.5E-15 0 2.94E-13 5.99E-14
AP mol H+ eq 1.92E-02 2.03E-04 1.41E-03 0 6.29E-04 0 4.29E-05 0 6.48E-04 8.71E-05
EP-
kg P eq 1.76E-05 5.89E-07 1.5E-05 0 1.4E-06 0 1.24E-07 0 4.08E-05 4.36E-08
freshwater
EP-marine kg N eq 5.18E-03 6.65E-05 3.44E-04 0 1.43E-04 0 1.4E-05 0 1.43E-04 2.96E-05
EP-terrestrial mol N eq 5.09E-02 7.92E-04 4.1E-03 0 1.48E-03 0 1.67E-04 0 1.57E-03 2.62E-04
kg NMVOC
POCP 1.64E-02 1.79E-04 1.19E-03 1.41E-05 3.82E-04 0 3.78E-05 0 4.62E-04 8.8E-05
eq
ADPE kg Sb eq 3.58E-06 1.65E-08 2.13E-07 0 7.8E-08 0 3.48E-09 0 1.52E-08 2.89E-09
ADPF MJ 1.88E+02 2.64E+00 1.12E+01 0 5.19E+00 0 5.57E-01 0 3.1E+00 7E-01
m3 world eq
WDP 1.23E+00 1.77E-03 1.35E-01 0 6.54E-02 0 3.74E-04 0 -2.16E-03 -1.6E-03
deprived
GWP = Global warming potential; ODP = Depletion potential of the stratospheric ozone layer; AP = Acidification potential of land and water; EP =
Eutrophication potential; POCP = Formation potential of tropospheric ozone photochemical oxidants; ADPE = Abiotic depletion potential for non-fossil
resources; ADPF = Abiotic depletion potential for fossil resources; WDP = Water (user) deprivation potential)
RESULTS OF THE LCA - INDICATORS TO DESCRIBE RESOURCE USE according to EN 15804+A2: 1 m² EcoWorx® Carpet (US
Made UK Market)
Parameter Unit A1-A3 A4 A5 B1 B2 C1 C2 C3 C4 D
PERE MJ 4.4E+00 1.58E-01 5.11E+00 0 2.88E+00 0 3.16E-02 0 2.55E-01 -2.86E-02
PERM MJ 5.31E+00 0 -4.19E+00 0 0 0 0 0 0 0
PERT MJ 9.7E+00 1.58E-01 9.18E-01 0 2.88E+00 0 3.16E-02 0 2.55E-01 -2.86E-02
PENRE MJ 1.54E+02 2.78E+00 1.53E+00 0 5.19E+00 0 5.58E-01 0 3.11E+00 7E-01
PENRM MJ 4.8E+01 0 -3.17E-01 0 0 0 0 0 0 0
PENRT MJ 2.01E+02 2.78E+00 1.21E+00 0 5.19E+00 0 5.58E-01 0 3.11E+00 7E-01
SM kg 1.47E+00 0 7.73E-02 0 0 0 0 0 0 -1.55E+00
RSF MJ 0 0 0 0 0 0 0 0 0 0
NRSF MJ 0 0 0 0 0 0 0 0 0 0
FW m3 3.7E-02 1.69E-04 1E-02 0 2.75E-03 0 3.58E-05 0 4.02E-05 8.16E-06
PERE = Use of renewable primary energy excluding renewable primary energy resources used as raw materials; PERM = Use of renewable primary
energy resources used as raw materials; PERT = Total use of renewable primary energy resources; PENRE = Use of non-renewable primary energy
excluding non-renewable primary energy resources used as raw materials; PENRM = Use of non-renewable primary energy resources used as raw
materials; PENRT = Total use of non-renewable primary energy resources; SM = Use of secondary material; RSF = Use of renewable secondary fuels;
NRSF = Use of non-renewable secondary fuels; FW = Use of net fresh water
RESULTS OF THE LCA – WASTE CATEGORIES AND OUTPUT FLOWS according to EN 15804+A2:
1 m² EcoWorx® Carpet (US Made UK Market)
Parameter Unit A1-A3 A4 A5 B1 B2 C1 C2 C3 C4 D
HWD kg 8.45E-09 1.27E-11 2.88E-09 0 4.49E-10 0 2.67E-12 0 4.79E-10 8.47E-11
NHWD kg 1.27E-01 3.79E-04 1.97E-01 0 4.77E-03 0 8E-05 0 3.07E+00 -3.4E-05
RWD kg 5.1E-03 3.25E-06 2.87E-04 0 8.3E-04 0 6.87E-07 0 3.81E-05 -7.64E-06
Environmental Product Declaration - Shaw Contract (Shaw Europe Ltd.) - EcoWorx® Carpet Tile (US Made UK Market) with EcoSolution Q®, Solution Q®, or Solution Q
5 Extreme® Face Fibre
CRU kg 0 0 0 0 0 0 0 0 0 0
MFR kg 0 0 1.81E-01 0 0 0 0 0 0 0
MER kg 0 0 0 0 0 0 0 0 0 0
EEE MJ 0 0 6.37E-02 0 0 0 0 0 0 0
EET MJ 0 0 9.77E-02 0 0 0 0 0 0 0
HWD = Hazardous waste disposed; NHWD = Non-hazardous waste disposed; RWD = Radioactive waste disposed; CRU = Components for re-use;
MFR = Materials for recycling; MER = Materials for energy recovery; EEE = Exported electrical energy; EET = Exported thermal energy
RESULTS OF THE LCA – additional impact categories according to EN 15804+A2-optional:
1 m² EcoWorx® Carpet (US Made UK Market)
Parameter Unit A1-A3 A4 A5 B1 B2 C1 C2 C3 C4 D
Disease
PM 1.52E-07 1.17E-09 1.28E-08 0 5.21E-09 0 2.48E-10 0 6.23E-09 9.27E-09
incidence
IR kBq U235 eq 4.29E-01 4.77E-04 2.51E-02 0 1.41E-01 0 1.01E-04 0 5.63E-03 4.81E-04
ETP-fw CTUe 8.35E+01 1.83E+00 5.38E+00 1.15E-04 2.35E+00 0 3.86E-01 0 3.04E+00 3.37E-01
HTP-c CTUh 2E-09 3.69E-11 1.4E-10 0 6.79E-11 0 7.79E-12 0 1.36E-10 1.06E-11
HTP-nc CTUh 6.64E-08 1.91E-09 5.56E-09 3.07E-12 2.65E-09 0 4.04E-10 0 1.14E-08 4.2E-10
SQP SQP 8.29E+00 9.07E-01 1.08E+01 0 1.87E+00 0 1.92E-01 0 2.23E-01 -5.6E-01
PM = Potential incidence of disease due to PM emissions; IR = Potential Human exposure efficiency relative to U235; ETP-fw = Potential comparative
Toxic Unit for ecosystems; HTP-c = Potential comparative Toxic Unit for humans (cancerogenic); HTP-nc = Potential comparative Toxic Unit for humans
(not cancerogenic); SQP = Potential soil quality index
Disclaimer 1: For the indicator 'Potential Human exposure efficiency relative to U235". This impact category deals mainly with the
eventual impact of low dose ionizing radiation on human health of the nuclear fuel cycle. It does not consider effects due to possible
nuclear accidents, occupational exposure nor due to radioactive waste disposal in underground facilities. Potential ionizing radiation
from the soil, from radon and from some construction materials is also not measured by this indicator.
Disclaimer 2: For the indicators 'Abiotic depletion potential for non-fossil resources', 'Abiotic depletion potential for fossil resources”,
“Water (user) deprivation potential", "Deprivation-weighted water consumption”, “Potential comparative toxic unit for ecosystems”,
“Potential comparative toxic unit for humans - cancerogenic”, “Potential comparative toxic unit for humans - non-carcinogenic”,
“Potential soil quality index”. The results of these environmental impact indicators shall be used with care as the uncertainties on these
results are high or as there is limited experienced with the indicators. This EPD was created using a software tool.
References
STANDARDS: ISO 15686-2:2011, Building and constructed assets — Service
life planning — Part 2: Service life prediction procedures.
EN 10874
EN 10874:2009, Resilient, textile and laminate floor coverings ISO 15686
— Classification. ISO 15686-7:2011, Building and constructed assets — Service
life planning — Part 7: Performance evaluation for feedback of
EN 1307 service life data from practice.
EN 1307:2014, Textile floor coverings — Classification.
ISO 15686
EN 14041 ISO 15686-8:2011, Building and constructed assets — Service
EN 14041:2004/AC:2006 — Resilient, textile and laminate floor life planning — Part 8: Reference service life and service life
coverings — Essential characteristics. estimation.
EN 15804 FURTHER REFERENCES:
EN 15804:2012+A2:2019/AC:2021, Sustainability of
construction works — Environmental product declarations — Candidate list
Core rules for the product category of construction products. Candidate List of substances of very high concern for
Authorisation, published on ECHA website, latest version
ISO 14025 17.01.2023 (https://echa.europa.eu/candidatelist-table).
ISO 14025:2011, Environmental labels and declarations —
Type III environmental declarations — Principles and Deutsche Umwelthilfe
procedures. Deutsche Umwelthilfe. Swept under the Carpet: The Big Waste
Problem of the Carpet Industry in Germany, 2017.
ISO 14040
ISO 14040:2006, Environmental management — Life cycle Envision LCA Tool
assessment — Principles and framework. Envision LCA Tool, 2021, Sphera Solutions GmbH, Leinfelden-
Echterdingen, with acknowledgement of LBP University of
ISO 14044 Stuttgart, version 1.
ISO 14044:2006, Environmental management — Life cycle
assessment — Requirements and guidelines. GaBi
GaBi Software System and Database for Life Cycle
ISO 15686 Engineering, 1992-2021, Sphera Solutions GmbH, Leinfelden-
ISO 15686-1:2011, Building and constructed assets — Service Echterdingen, with acknowledgement of LBP University of
life planning — Part 1: General principles and framework. Stuttgart, program version GaBi 10; database version 2021.1.
ISO 15686 GaBi documentation
Environmental Product Declaration - Shaw Contract (Shaw Europe Ltd.) - EcoWorx® Carpet Tile (US Made UK Market) with EcoSolution Q®, Solution Q®, or Solution Q
6 Extreme® Face Fibre
GaBi dataset documentation for the software system and Umwelt e.V., 2021.
databases, LBP, University of Stuttgart and Sphera Solutions
GmbH, Leinfelden-Echterdingen, 2021 (http://www.gabi- PCR Part B
software.com/support/gabi/gabi-database-2021-lci- Product Category Rules for Building Products, Part B:
documentation/). Requirements on the EPD for floor coverings, version 1.7, 2022
(www.bau-umwelt.de).
IBU 2021
Institut Bauen und Umwelt e.V.: General Instructions for the Packaging disposal rates
EPD programme of Institut Bauen und Umwelt e.V., Version Eurostat, Recovery and recycling rates for packaging. 2015
2.0, Berlin: Institut Bauen und Umwelt e.V., 2021 (www.ibu- (http://ec.europa.eu/eurostat/web/environment/waste/main-
epd.com). tables).
The literature referred to in the Environmental Product
PCR Part A Declaration must be listed in full.Standards already fully quoted
PCR Part A: Calculation rules for the Life Cycle Assessment in the EPD do not need to be listed here again.
and Requirements on the Background Report according to EN The current version of PCR Part A and PCR Part B of the PCR
15804:2012+A2:2019/AC:2021, Version 1.3, Institut Bauen und document on which they are based must be referenced.
Environmental Product Declaration - Shaw Contract (Shaw Europe Ltd.) - EcoWorx® Carpet Tile (US Made UK Market) with EcoSolution Q®, Solution Q®, or Solution Q
7 Extreme® Face Fibre
Publisher
Institut Bauen und Umwelt e.V. +49 (0)30 3087748- 0
Hegelplatz 1 info@ibu-epd.com
10117 Berlin www.ibu-epd.com
Germany
Programme holder
Institut Bauen und Umwelt e.V. +49 (0)30 3087748- 0
Hegelplatz 1 info@ibu-epd.com
10117 Berlin www.ibu-epd.com
Germany
Author of the Life Cycle Assessment
Sphera Solutions GmbH +49 711 341817-0
Hauptstraße 111- 113 info@sphera.com
70771 Leinfelden-Echterdingen www.sphera.com
Germany
Owner of the Declaration
Shaw Contract (Shaw Europe Ltd.) +1 800 257 7429
Blackaddie Road * infouk@shawcontract.com
DG46DB Sanquhar www.shawcontract.com
United Kingdom
Environmental Product Declaration - Shaw Contract (Shaw Europe Ltd.) - EcoWorx® Carpet Tile (US Made UK Market) with EcoSolution Q®, Solution Q®, or Solution Q
8 Extreme® Face Fibre
