ENVIRONMENTAL PRODUCT DECLARATION
as per ISO 14025 and EN 15804+A2
Owner of the Declaration Stiferite
Publisher Institut Bauen und Umwelt e.V. (IBU)
Programme holder Institut Bauen und Umwelt e.V. (IBU)
Declaration number EPD-STF-20220334-CBC2-EN
Issue date 16.02.2023
Valid to 15.02.2028
Stiferite RP average thick panel
Stiferite
www.ibu-epd.com | https://epd-online.com
General Information
Stiferite Stiferite RP average thick panel
Programme holder Owner of the declaration
IBU – Institut Bauen und Umwelt e.V. Stiferite
Hegelplatz 1 Viale Navigazione Interna 54
10117 Berlin 35129 Padova
Germany Italy
Declaration number Declared product / declared unit
EPD-STF-20220334-CBC2-EN Stiferite RP consists of a polyiso (PIR) rigid foam panel, covered with multi-
layer gas diffusion tight facers on both sides and integrated vapour barrier
on the hot side, bonded to a 13 mm plasterboard (CG), and produced by
Stiferite. The EPD applies to 1 m2 of 77.8 mm thick PUR sandwich board,
i.e. 0.0778 m3, with an average density between foam and facing of 153
kg/m3.
This declaration is based on the product category rules: Scope:
Insulating materials made of foam plastics, 01.08.2021 Stiferite produces Stiferite RP that is a high performance insulation board
(PCR checked and approved by the SVR) manufactured from closed cell expanded rigid polyurethane foam, covered
on both sides with multi-layer gas diffusion tight facers and integrated
vapour barrier on the hot side, bonded to a 13 mm plasterboard. The data
Issue date have been provided by the only Stiferite factory that is located in Padova
(Italy) for the year 2021 and sold worldwide.
16.02.2023
The owner of the declaration shall be liable for the underlying information
and evidence; the IBU shall not be liable with respect to manufacturer
information, life cycle assessment data and evidences.
Valid to
15.02.2028 The EPD was created according to the specifications of EN 15804+A2. In
the following, the standard will be simplified as EN 15804.
Verification
The standard EN 15804 serves as the core PCR
Independent verification of the declaration and data according to ISO
14025:2011
internally X externally
Dipl.-Ing. Hans Peters
(Chairman of Institut Bauen und Umwelt e.V.)
Dipl.-Ing. Hans Peters Prof. Dr. Birgit Grahl,
(Managing Director Institut Bauen und Umwelt e.V.) (Independent verifier)
1 Environmental Product Declaration - Stiferite - Stiferite RP average thick panel
Product
Union/European Free Trade Association (EU/EFTA) (with the
Product description/Product definition exception of Switzerland) Regulation (EU) No.305/2011 (CPR)
Stiferite's thermal insulation panels are mainly used in the applies. The product needs a Declaration of Performance
building/construction sector and in industrial insulation. taking into consideration EN 13950:2014 Gypsum board
The panels are made of thermo-setting closed cells thermal/acoustic insulation composite - Definitions,
polyurethane foam (PU) supplied with various types of flexible requirements and test methods and the CE-marking.
facers on both sides of the panel. The nature/type of facer is a For the application and use the respective national provisions
function of the type of panel and its application. apply.
Expanded rigid polyurethane foam is distinguished by its
thermal insulation performance, mechanical resistance, Base materials/Ancillary materials
workability, lightness, and durability. Core material (about 17.1 % of the weight of the declared
The performance of Stiferite's panels is determined based on unit):
the European norm EN13165:2012+A2:2016 Thermal
insulation products for buildings - Factory-made rigid Closed-cell Polyiso (PIR) rigid foam made from MDI (50-65 %),
polyurethane foam (PU) products - Specification. polyols (20-30 %), pentane (4-6 %) and additives (4-6 %).
The performance of Stiferite's composite panels is determined
based on the European norm EN 13950:2014 Gypsum board Facing (about 1.3 % of the weight of the declared unit): multi-
thermal/acoustic insulation composite - Definitions, layer gas diffusion tight facers consisting of PE (10-20 %),
requirements and test methods. aluminium (15-25 %), and paper (60-70 %).
This EPD refers to Stiferite's RP average thick panel, made of Additional panel (about 81.6 % of the weight of the declared
an insulation component in polyurethane foam using blowing unit): plasterboard (95-99 %) and glue (1-2 %).
agent Pentanebased, covered on both side with multi-facer gas
diffusion tight and integrated vapour barrier on the hot side, The PU board for insulation:
bonded to a 13 mm plasterboard. and bonded to one side with
• This product/article/at least one partial article contains
13 mm thick plasterboard. The properties of Stiferite RP panel
substances listed in the candidate list (date: 17.01.2022)
components ensure excellent reaction to fire (European B-
exceeding 0.1 percentage by mass: no
s1,d0 class) The panel is produced in standard dimensions of
1200 x 3000 mm and straight finish borders. • This product/article/at least one partial article doesn't
Upon request and for minimum quantities, the panels may be contain other carcinogenic, mutagenic, reprotoxic
produced in various dimensions, and the borders may be (CMR) substances in categories 1A or 1B which are not
rabbeted along the sides. The surface of the panel may be on the candidate list, exceeding 0.1 percentage by
evened out with sandpaper in order to allow installation on mass: no
uneven surfaces. Stiferite RP panel is produced by a certified • Biocide products were added to this construction
company with systems:ISO 9001, ISO 45001, ISO 14001 in its product or it has been treated with biocide products (this
entire line of products. then concerns a treated product as defined by the (EU)
Ordinance on Biocide Products No.528/2012): no
Application
Additional declaration according to quoted law: The product is
The Stiferite RP panel is suitable for insulating. Walls and compliant with all requirements indicated in chapter 2.5.7
Ceilings applications from the inside. 'Isolanti termici ed acustici' of the n.256 D.L. of the 23th June
2022 (CAM EDILIZIA):
Technical Data
In this Life Cycle Assessment, a PU insulation board with the • Any blowing agent with Ozone depletion potential >0 is
following properties has been regarded: not used in production
• Any substances of Very High Concern-SVHC in
Constructional data
concentration of more than 0,1 %w are not used in
Name Value Unit production (REACH n. 1907/2006). Any specific
Gross density 153 kg/m3 authorizations for use are eserved provided for by the
same Regulation for the substances included in Annex
Declared Average Thermal Resistance RD acc.
3.01 m²K/W XIV and specifications restrictions set out in Annex XVII
to EN 13165
of the Regulation.
Compressive strength at 10% deformation acc.
>150 kPa • Catalysts lead-based are not used in production
to EN 826
• Flame retardants used in production (belonging to the
Tensile strength perpendicular to the face acc. >30 kPa Organophosphorus class) are not banned by any
to EN 1607 national or European regulation
Water absorption by total immersion acc. to EN • According to the raw materials declarations of suppliers,
<1 Vol.-%
12087 the minimum amount of recycled raw materials based
Water absorption by partial immersion acc. to on the insulation board (PU foam and facers) weight is 3
< 0.1 kg/m²
EN 1609 % w and the minimum amount of recycled raw materials
Water vapour diffusion resistance factor μ acc. 89900 based on the PU insulation foam weight is 4 % w in
to EN 12086 compliance with REMADE in Italy type 1 certification
B- (note: this information is not explicitly considered in the
Euroclass reaction to fire acc. to EN 11925
s1,d0 LCA and not included in the EPD tables that only refer
to recycling content in the foreground system).
This provides a thermal resistance R = 3.01 m² k/W.
Reference service life
Product according to the CPR based on a EN/:13950:2014 For
The durability of insulation panels is normally at least as long as
the placing on the market of the product in the European
the lifetime of the building in which it is used. The experimental
2 Environmental Product Declaration - Stiferite - Stiferite RP average thick panel
data show that the reference life is greater than 50 years.
LCA: Calculation rules
Declared Unit A1 - Raw material formulation
The declared unit is 1 m² with a thickness of 77.8 mm, e. g. A2 - Raw material transport
0.0778 m³. A3 - Production of the insulation board and packaging material
Corresponding conversion factors are listed in the table below. A4 - Transport to the construction site
Declared unit C1 - demolition and deconstruction
C2 - Transport to end of life
Name Value Unit
C3 - End-of-Life: waste management (thermal recovery)
Declared unit 1 m2 C4 - End-of-Life: waste management (landfill)
Gross density 153 kg/m3 D - Benefits and loads beyond system boundary
Grammage 11.9 kg/m2
Geographic Representativeness
Layer thickness 0.0778 m
Land or region, in which the declared product system is
Declared average thermal resistnace RD 3.01 m²K/W manufactured, used or handled at the end of the product´s
lifespan: Italy
This provides a thermal resistance R = 3.01 m² /W.
Comparability
System boundary
Basically, a comparison or an evaluation of EPD data is only
Type of the EPD: cradle to gate - with options This life cycle
possible if all the data sets to be compared were created
assessment for the production of the polyurethane insulation
according to EN 15804 and the building context, respectively
board considers the life cycle from the supply of raw materials
the product-specific characteristics of performance, are taken
to the manufacturer´s gate (cradle-to-gate with options). It also
into account. The background database used is GaBi 2022
includes the transport to the construction site and the end-of-life
database (v. 2022.1)
stage of the used PU thermal insulation board. The life cycle is
split into the following individual phases:
LCA: Scenarios and additional technical information
End of life (C1-C4)
Characteristic product properties of biogenic carbon
Name Value Unit
Information on describing the biogenic Carbon Content at
Scenario No 1: Material Incineration 100 %
factory gate
Scenario No 2: Landfill 100 %
Name ValueUnit
kg C1 – Deconstruction and demolition (0.2 MJ/kg as electrical
Biogenic carbon content in product 0.043 C consumption assumed)
Biogenic carbon content in accompanying kg
0.003 C2 – Panel is transported from the building site to a treatment
packaging C
plant by truck and an average distance of 100 km is
considered.
Transport to the building site (A4) C3/C4- Disposal scenarios used are divided into 2 sub-
scenarios:
Name ValueUnit
1) Incineration 100 % (C3/1)
Truck with a capacity of 17.3 tons 252 km
2) Landfilling 100 % (C4/2)
Ferry with a capacity of 1200-10000 dwt payload
0.703 km
capacity
Reuse, recovery and/or recycling potentials (D), relevant
Ship with a capacity of 27500 dwt payload capacity 0 km scenario information
tons
D: Benefits and loads beyond system boundary are divided into
Plane with a capacity of 22 ton 0 km 2 sub-scenarios:
Name Value Unit
Type and amount of packaging included in module A3
Scenario No 1: Material Incineration 100 %
Name Value Unit
Scenario No 2: Landfill 100 %
Cardboard 0.00691 kg
EPS stock 0.00578 kg
EPS stock - glue 0.00041 kg
Paper labels 0.00014 kg
PE film 0.04031 kg
PP tape 0.00005 kg
PUR stucks 0 kg
SBR labels 0.00001 kg
TOTAL PACKAGING 0.05362 kg
3 Environmental Product Declaration - Stiferite - Stiferite RP average thick panel
LCA: Results
The tables below show the results of the LCA. Basic information on all declared modules provides chapter 4.
There are two scenarios for the end-of-life (C2, C4 and D) analyzed: Scenario 1 considers 100 % incineration, Scenario 2 considers
100 % landfill disposal.
For SM, RSF, NRSF, CRU indicators only the foreground system is considered.
DESCRIPTION OF THE SYSTEM BOUNDARY (X = INCLUDED IN LCA; ND = MODULE OR INDICATOR NOT DECLARED; MNR =
MODULE NOT RELEVANT)
Benefits and
Construction loads beyond
Product stage Use stage End-of-life stage
process stage the system
boundaries
la ire ta m w a Ry lp p u s tro p s n a rT g n iru tc a fu n a M e h t m o rf tro p s n a rTe tis e h t o t e ta g y lb m e s s A e s U e c n a n e tn ia M ria p e R tn e m e c a lp e R tn e m h s ib ru fe R y g re n e la n o ita re p Oe s u re ta w la n o ita re p Oe s u n o itc u rts n o c -e Dn o itilo m e d tro p s n a rT g n is s e c o rp e ts a W la s o p s iD -e s u e R-y re v o c e R-g n ilc y c e Rla itn e to p
A1 A2 A3 A4 A5 B1 B2 B3 B4 B5 B6 B7 C1 C2 C3 C4 D
X X X X MND MND MND MNR MNR MNR MND MND X X X X X
RESULTS OF THE LCA - ENVIRONMENTAL IMPACT according to EN 15804+A2: 1 m2 Stiferite RP
Parameter Unit A1-A3 A4 C1 C2 C3/1 C3/2 C4/1 C4/2 D/1 D/2
GWP-total kg CO 2 eq 7.91E+00 2.55E-01 2.72E-01 7.2E-02 6E+00 0 0 3.32E-01 -2.26E+00 0
GWP-fossil kg CO 2 eq 8.7E+00 2.53E-01 2.72E-01 7.13E-02 5.87E+00 0 0 1.9E-01 -2.25E+00 0
GWP-
biogenic kg CO 2 eq -7.94E-01 8.22E-04 1.6E-04 2.31E-04 1.39E-01 0 0 1.42E-01 -2.07E-03 0
GWP-luluc kg CO 2 eq 3.63E-03 1.7E-03 1.76E-05 4.79E-04 4.9E-04 0 0 3.28E-04 -1.2E-04 0
ODP kg CFC11 eq 1.61E-11 2.49E-14 2.68E-12 6.99E-15 5.93E-12 0 0 4.3E-13 -1.62E-11 0
AP mol H+ eq 1.42E-02 9.05E-04 3.99E-04 2.38E-04 5.37E-03 0 0 1.29E-03 -2.75E-03 0
EP-
kg P eq 2.74E-05 9.04E-07 1.22E-07 2.54E-07 3.11E-06 0 0 2.75E-06 -7.71E-07 0
freshwater
EP-marine kg N eq 4.19E-03 4.17E-04 1.09E-04 1.09E-04 2.33E-03 0 0 3.41E-04 -8.06E-04 0
EP-terrestrial mol N eq 4.29E-02 4.67E-03 1.16E-03 1.22E-03 2.61E-02 0 0 3.65E-03 -8.67E-03 0
kg NMVOC
POCP 1.62E-02 8.17E-04 3.08E-04 2.13E-04 6.12E-03 0 0 1.05E-03 -2.3E-03 0
eq
ADPE kg Sb eq 3.53E-06 2.55E-08 3.23E-08 7.17E-09 1.24E-07 0 0 1.89E-08 -2.24E-07 0
ADPF MJ 1.95E+02 3.33E+00 5.76E+00 9.34E-01 1.96E+01 0 0 2.5E+00 -4.46E+01 0
m3 world eq
WDP 1.58E+00 2.83E-03 2.03E-02 7.96E-04 1.63E+00 0 0 1.95E-02 -1.24E-01 0
deprived
GWP = Global warming potential; ODP = Depletion potential of the stratospheric ozone layer; AP = Acidification potential of land and water; EP =
Eutrophication potential; POCP = Formation potential of tropospheric ozone photochemical oxidants; ADPE = Abiotic depletion potential for non-fossil
resources; ADPF = Abiotic depletion potential for fossil resources; WDP = Water (user) deprivation potential)
RESULTS OF THE LCA - INDICATORS TO DESCRIBE RESOURCE USE according to EN 15804+A2: 1 m2 Stiferite RP
Parameter Unit A1-A3 A4 C1 C2 C3/1 C3/2 C4/1 C4/2 D/1 D/2
PERE MJ 2.09E+01 2.3E-01 8.32E-01 6.47E-02 4.31E+00 0 0 2.05E+00 -5.05E+00 0
PERM MJ 1.81E+00 ND ND ND -1.69E+00 0 0 -1.69E+00 ND 0
PERT MJ 2.28E+01 2.3E-01 8.32E-01 6.47E-02 2.62E+00 0 0 3.6E-01 -5.05E+00 0
PENRE MJ 1.05E+02 3.34E+00 5.76E+00 9.37E-01 1.08E+02 0 0 9.05E+01 -4.46E+01 0
PENRM MJ 9.02E+01 ND ND ND -8.8E+01 0 0 -8.8E+01 ND 0
PENRT MJ 1.95E+02 3.34E+00 5.76E+00 9.37E-01 1.96E+01 0 0 2.5E+00 -4.46E+01 0
SM kg 2.38E-01 ND ND ND ND 0 0 ND ND 0
RSF MJ ND ND ND ND ND 0 0 ND ND 0
NRSF MJ ND ND ND ND ND 0 0 ND ND 0
FW m3 5.16E-02 2.66E-04 1.26E-03 7.48E-05 3.98E-02 0 0 5.94E-04 -7.67E-03 0
PERE = Use of renewable primary energy excluding renewable primary energy resources used as raw materials; PERM = Use of renewable primary
energy resources used as raw materials; PERT = Total use of renewable primary energy resources; PENRE = Use of non-renewable primary energy
excluding non-renewable primary energy resources used as raw materials; PENRM = Use of non-renewable primary energy resources used as raw
materials; PENRT = Total use of non-renewable primary energy resources; SM = Use of secondary material; RSF = Use of renewable secondary fuels;
NRSF = Use of non-renewable secondary fuels; FW = Use of net fresh water
RESULTS OF THE LCA – WASTE CATEGORIES AND OUTPUT FLOWS according to EN 15804+A2:
1 m2 Stiferite RP
Parameter Unit A1-A3 A4 C1 C2 C3/1 C3/2 C4/1 C4/2 D/1 D/2
HWD kg 7.06E-08 1.77E-11 4.12E-10 4.96E-12 2.02E-09 0 0 1.52E-10 -4.29E-09 0
NHWD kg 7.35E-01 5.44E-04 1.22E-03 1.53E-04 4.36E+00 0 0 1.18E+01 -9.92E-03 0
RWD kg 2.46E-03 6.19E-06 9.57E-04 1.74E-06 1.57E-03 0 0 2.82E-05 -5.78E-03 0
CRU kg ND ND ND ND ND 0 0 ND ND 0
4 Environmental Product Declaration - Stiferite - Stiferite RP average thick panel
MFR kg ND ND ND ND ND 0 0 ND ND 0
MER kg ND ND ND ND ND 0 0 ND ND 0
EEE MJ ND ND ND ND 1.45E+01 0 0 4.07E-02 ND 0
EET MJ ND ND ND ND 9.05E+00 0 0 ND ND 0
HWD = Hazardous waste disposed; NHWD = Non-hazardous waste disposed; RWD = Radioactive waste disposed; CRU = Components for re-use;
MFR = Materials for recycling; MER = Materials for energy recovery; EEE = Exported electrical energy; EET = Exported thermal energy
RESULTS OF THE LCA – additional impact categories according to EN 15804+A2-optional:
1 m2 Stiferite RP
Parameter Unit A1-A3 A4 C1 C2 C3/1 C3/2 C4/1 C4/2 D/1 D/2
Disease
PM 1.67E-07 5.32E-09 3.56E-09 1.36E-09 5.55E-08 0 0 1.57E-08 -2.44E-08 0
incidence
IR kBq U235 eq 3.09E-01 9.35E-04 1.4E-01 2.63E-04 2.33E-01 0 0 3.24E-03 -8.45E-01 0
ETP-fw CTUe 7.67E+01 2.36E+00 1.76E+00 6.62E-01 6.96E+00 0 0 4.16E+01 -1.07E+01 0
HTP-c CTUh 4.62E-09 4.86E-11 3.25E-11 1.36E-11 2.59E-10 0 0 2.04E-10 -2.72E-10 0
HTP-nc CTUh 3.92E-07 3.02E-09 1.65E-09 8.36E-10 1.67E-08 0 0 2.25E-08 -1.31E-08 0
SQP SQP 4.43E+01 1.41E+00 5.28E-01 3.95E-01 2.7E+00 0 0 4.89E-01 -3.21E+00 0
PM = Potential incidence of disease due to PM emissions; IR = Potential Human exposure efficiency relative to U235; ETP-fw = Potential comparative
Toxic Unit for ecosystems; HTP-c = Potential comparative Toxic Unit for humans (cancerogenic); HTP-nc = Potential comparative Toxic Unit for humans
(not cancerogenic); SQP = Potential soil quality index
Disclaimer 1 – for the indicator “Potential Human exposure efficiency relative to U235”. This impact category deals mainly with the
eventual impact of low-dose ionizing radiation on human health of the nuclear fuel cycle. It does not consider effects due to possible
nuclear accidents, occupational exposure or radioactive waste disposal in underground facilities. Potential ionizing radiation from the
soil, radon and from some construction materials is also not measured by this indicator.
Disclaimer 2 – for the indicators “abiotic depletion potential for non-fossil resources”, “abiotic depletion potential for fossil resources”,
“water (user) deprivation potential, deprivation-weighted water consumption”, “potential comparative toxic unit for ecosystems”,
“potential comparative toxic unit for humans – cancerogenic”, “Potential comparative toxic unit for humans - not cancerogenic”,
“potential soil quality index”. The results of this environmental impact indicator shall be used with care as the uncertainties on these
results are high as there is limited experience with the indicator.
References
Standards CPR products -Specification
Regulation (EU) No.305/2011 laying down harmonised
conditions for the marketing of construction products and EN 13950
repealing Council Directive 89/106/EEC EN 13950:2014 Gypsum board thermal/acoustic insulation
composite - Definitions, requirements and test methods.
EN 826
EN 826:2013 Determination of Compression Behavior of EN 15804
Thermal Insulation Products EN 15804:2012+A2:2019+AC:2021 Sustainability of
construction works — Environmental Product Declarations —
EN 1607 Core rules for the product category of construction products.
EN 1607: 2013 Thermal insulating products for building
applications. Determination of tensile strength perpendicular to ISO 9001
faces ISO 9001:2015 Quality management
EN 1609 ISO 14001
EN 1609: Thermal insulating products for building applications. ISO 14001: 2015 Environmental management systems
Determination of short term water absorption by partial
immersion. ISO 14025
EN ISO 14025:2011 Environmental labels and declarations —
EN 11925 Type III environmental declarations - Principles and procedures.
EN 11925:2010 Reaction to fire tests. Ignitability of products
subjected to direct impingement of flame. Single-flame source ISO 45001
test. ISO 45001: 2018 Occupational health and safety management
systems
EN 12086
EN 12086: 2013 Thermal insulating products for building GaBi 2022
applications. Determination of water vapour transmission GaBi 10 and DB 2022.1: Documentation of GaBi 10: Software-
properties. System and Database for Life Cycle Engineering. Copyright,
TM. Stuttgart, Leinfelden-Echterdingen, 1992-2022
EN 12087 http://www.gabi-software.com
EN 12087:2013 Thermal insulating products for building
applications. Determination of long term water absorption by IBU 2021
immersion. Institut Bauen und Umwelt e.V.: General Instructions for the
EPD programme of Institut Bauen und Umwelt e.V., Version
EN 13165 2.0, Berlin: Institut Bauen und Umwelt e.V., 2021 www.ibu-
EN 13165:2012+A2:2016 Thermal insulation products for epd.com
buildings - Factory made rigid polyurethane foam (PU)
5 Environmental Product Declaration - Stiferite - Stiferite RP average thick panel
IBU PCR Part A Gazzetta Ufficiale della Repubblica Italiana, Serie Generale
Product Category Rules for Building-Related Products and n.183 del 06-08-2022 https://www.mite.gov.it/notizie/novita-sui-
Services. criteri-minini-ambientali-cam REACH REACH Registration,
Part A: Calculation Rules for the Life Cycle Assessment and Evaluation, Authorization and Restriction of Chemical, 2007
Requirements on the Project Report according to EN
15804+A2:2019; V1.2, 11/2021 Ordinance on Biocide Products
Regulation (eu) n. 528/2012 of the European Parliament and of
IBU PCR Part B the Council of 22 May 2012 concerning the making available on
PCR Guidance-Texts for Building-Related Products and the market and use of biocidal products Text with EEA
Services; Part B: Requirements on the EPD for Insulating relevance
materials made of foam plastics; Institute Construction and
Environment e.V. (IBU). Version 01.2019 https://epd-online.com REMADE IN ITALY
Certificate No.1245/001 for Stiferite Rev. n. 0 18 November
PANGPP 2022 2021
Piano d' Azione Nazionale sul Green Public Procurement
(PANGPP) – Decreto Ministeriale n. 256 del 23-06-2022 STIFERITE LCA tool background report v 2.3 (03-06-2022)
6 Environmental Product Declaration - Stiferite - Stiferite RP average thick panel
Publisher
Institut Bauen und Umwelt e.V. +49 (0)30 3087748- 0
Hegelplatz 1 info@ibu-epd.com
10117 Berlin www.ibu-epd.com
Germany
Programme holder
Institut Bauen und Umwelt e.V. +49 (0)30 3087748- 0
Hegelplatz 1 info@ibu-epd.com
10117 Berlin www.ibu-epd.com
Germany
Author of the Life Cycle Assessment
Sphera Solutions GmbH +49 711 341817-0
Hauptstraße 111- 113 info@sphera.com
70771 Leinfelden-Echterdingen www.sphera.com
Germany
Owner of the Declaration
Stiferite +39 049 8997911
Viale Navigazione Interna 54 info@stiferite.com
35129 Padova www.stiferite.com
Italy
7 Environmental Product Declaration - Stiferite - Stiferite RP average thick panel
