ENVIRONMENTAL PRODUCT DECLARATION
as per ISO 14025 and EN 15804+A2
Owner of the Declaration VELUX Group
Publisher Institut Bauen und Umwelt e.V. (IBU)
Programme holder Institut Bauen und Umwelt e.V. (IBU)
Declaration number EPD-VEL-20240209-IBA1-EN
Issue date 23.07.2024
Valid to 22.07.2029
VELUX Commercial Polycarbonate rooflights (PC-ovenlys)
VELUX Group
www.ibu-epd.com | https://epd-online.com
1. General Information
VELUX Group VELUX Commercial Polycarbonate rooflights (PC-
ovenlys)
Programme holder Owner of the declaration
IBU – Institut Bauen und Umwelt e.V. VELUX Group
Hegelplatz 1 Ådalsvej 99
10117 Berlin 2970 Hørsholm
Germany Denmark
Declaration number Declared product / declared unit
EPD­VEL­20240209­IBA1­EN 1 m2 of VELUX Commercial Polycarbonate rooflights (PC­ovenlys)
This declaration is based on the product category rules: Scope:
Windows and doors , 01.08.2021 The LCA represents 100% of the production volume of VELUX
(PCR checked and approved by the SVR) Commercial polycarbonate rooflights produced by VELUX Commerical in
Kongerslev (DK).
The owner of the declaration shall be liable for the underlying information
Issue date and evidence; the IBU shall not be liable with respect to manufacturer
information, life cycle assessment data and evidences.
23.07.2024
The EPD was created according to the specifications of EN 15804+A2. In
the following, the standard will be simplified as EN 15804.
Valid to
22.07.2029 Verification
The standard EN 15804 serves as the core PCR
Independent verification of the declaration and data according to ISO
14025:2011
internally X externally
Dipl.­Ing. Hans Peters
(Chairman of Institut Bauen und Umwelt e.V.)
Florian Pronold Dr.­Ing. Nikolay Minkov,
(Managing Director Institut Bauen und Umwelt e.V.) (Independent verifier)
1 Environmental Product Declaration ­ VELUX Group ­ VELUX Commercial Polycarbonate rooflights (PC­ovenlys)
2. Product
• EN 1873:2005, Prefabricated accessories for roofing -
2.1 Product description/Product definition
Individual rooflights of plastics - Product specification
Polycarbonate rooflights (PC­ovenlys) are 10, 20 or 30 mm
and test methods.
polycarbonate multiwall rooflights in either vaulted, flat or ridge
shape. The outer layer is made in acrylic (PMMA) or 2.4 Delivery status
polycarbonate material.The upstand is made of either insulated
VELUX Commercial polycarbonate rooflights are avilable in
plywood put together in a sandwich construction or as massive
sizes ranging from 600 mm x 900 mm (0.48 m2) to 2400 mm x
rafter wood.
4800 mm (11.52 m2) with a standard size of 1200 mm x 2400
mm (2.88 m2). The height can range from 100 mm to 1000 mm
For the placing on the market of the product in the European
with a standard height of 300 mm.
Union/European Free Trade Association (EU/EFTA) (with the
exception of Switzerland) Regulation (EU) No. 305/2011 (CPR)
2.5 Base materials/Ancillary materials
applies. The product needs a declaration of performance taking
The delcared product is composed of:
into consideration:
Name Value Unit
• EN 1873:2005, Prefabricated accessories for roofing -
Sawn timber 32 % ­
Individual rooflights of plastics - Product specification
and test methods plywood 30 % ­
and the CE­marking. Polycarbonate (PC) 16 % ­
Stone wool 7% ­
2.2 Application
Rubber 3 %
VELUX Commercial polycarbonate rooflights are intended for
Steel 2 %
lighting by means of daylight and of ventilating interior spaces
by means of opening devices. Others 2 % ­
Areas of application for the VELUX Commercial polycarbonate
rooflights (PC­ovenlys) are:
1. This product/article/at least one partial article contains
• unheated industrial buildings substances listed in the ECHA candidate list (date: 15.08.2023)
• heated industrial buildings exceeding 0.1 percentage by mass: no.
• warehouses
• sports halls railway stations 2. This product/article/at least one partial article contains other
carcinogenic, mutagenic or reprotoxic (CMR) substances in
2.3 Technical Data categories 1A or 1B which are not on the ECHA candidate list,
Technical characteristics exceeding 0.1 percentage by mass: not investigated with
suppliers.
Technical characteristics according to DoP No. 457501-2a for
polycarbonate rooflight, Type HV10. HV20. HV30.
3. Biocide products were added to this construction product or it
HV30+/RY10. RY20. RY30/PL10. PL20. PL30 + with or without
has been treated with biocide products (this then concerns a
upstand
treated product as defined by the (EU) Ordinance on Biocide
Name Value Unit
Products No. 528/2012): no.
Restistance to upward load NPD
2.6 Manufacture
Resistance to downward load NPD
All the raw materials including wood, plywood, polycarbonate,
Durability NPD
acrylic, aluminium, actuators and all ancillary materials (fittings,
Air permeability NPD
screws, glue, plastic parts, gasket, etc.) are bought from
Direct airborne sound insulation acc. EN NPD / 20 ­ 23 dB external suppliers. First the wood and plywood are cross­cut for
1873 the production of the upstands; in addition, all aluminium parts
Thermal transmittance acc. EN 1873 1.2­1.9 are cross­cut, drilled and welded; in a last preparatory step, the
Luminous transmittance (clear) acc. EN NPD / 35 % ­ 74 polycarbonate and the acrylic are crosscut and shaped. All the
1873 % components are then assembled to the final product, which
undergoes a final inspection.
Luminous transmittance (opal) acc. EN NPD / 29 % ­ 60
Only a few items are bought manufactured from a sub supplier.
1873 %
That is the aluminium sheets for windscreens and standard
Reaction to fire, wooden frame acc. EN
D­s2, d0 sizes frames for insulated upstands. Also the wood for solid
13501
frames (Kehlet) is bought from external.
Reaction to fire, top plate acc. EN 13501 B­s1, d0
Normally aluminium is not surface treated; sometimes the
Resistance to fire NPD aluminium parts are painted (wet paint) from a local dealer, but
External fire performance NPD not very often.
Water tightness NPD The insulated upstand made from wood/plywood come usually
as laminated material; only in a few cases, the interior side of
Small, hard body NPD
the upstands are painted.
Large, soft body EN 1873 NPD / SB 600
In order to guarantee the quality assurance of the product,
NPD: no performance declared VELUX operates a quality management system according to
ISO 9001.
Performance data of the product in accordance with the
2.7 Environment and health during manufacturing
declaration of performance with respect to its essential
characteristics according to: The health of employees is protected by suitable measures
specified by the authorities. These include safety goggles,
2 Environmental Product Declaration ­ VELUX Group ­ VELUX Commercial Polycarbonate rooflights (PC­ovenlys)
hearing protection, helmets, gloves, safety shoes, etc.
Waste generated during every process in the company is 2.13 Extraordinary effects
collected, sorted and disposed of in a professional and Fire
resource­conserving manner. See table 2.3 for the reaction to fire of the different
components.
2.8 Product processing/Installation
The rooflights upstand is fixed to the roof sub­construction with Water
screws and brackets (not supplied by VELUX Commercial). The In the event of unforeseen exposure to water (flood), no
type of fastening depends on the sub­construction. After fixating adverse effects on human health or the environment are to be
the upstand, the factory pre­assembled top unit is fixed to the expected.
upstand or ventilation frame using screws.
After fixating the complete rooflight, the roof membrane is Mechanical destruction
sealed with materials brought by the installer. In the event of unforeseen mechanical destruction, VELUX
Commercial polycarbonate rooflights must be replaced; no
2.9 Packaging adverse effects on human health or the environment are to be
For the transport to the construction site, the VELUX expected.
Commercial polycarbonate rooflights are loaded onto a lorry
and fixed with multi­use fastening belts. Usually, no additional 2.14 Re-use phase
packaging is used. VELUX commercial polycarbonate rooflights can be dismantled
manually without any problems. The metal parts are usually
2.10 Condition of use recycled, and the wooden and plastic parts are sent for thermal
The material composition of VELUX Commercial polycarbonate recycling for energy recovery.
rooflights do not change over their service life.
2.15 Disposal
2.11 Environment and health during use VELUX Commercial polycarbonate rooflights can be disposed
VELUX Commercial polycarbonate rooflights do not contain any of in an appropriate landfill. However, due to the value of the
pollutants that could be released during use. materials or the carbon content of the wooden and plastic parts,
recycling or energy recovery is preferable and common.
Environmental protection: According to current knowledge,
hazards to water, air and soil cannot arise when the products Waste code according to the European Waste List (Regulation
are used as intended. on the European Waste List):
17 02 01 wood
Health protection: According to current knowledge, no health 17 02 03 plastics
hazards or impairments are to be expected. 17 04 02 aluminium
17 04 05 iron and steel
2.12 Reference service life
It is not possible to calculate the reference service life 2.16 Further information
according to ISO 15686. The service life based on a Further documentation on the products, technical data sheets,
manufacturer's declaration is 30 years. The corresponding BIM files, etc. can be found at:
utilization scenario is declared in chapter 4.
www.commercial.velux.com
3. LCA: Calculation rules
an R­value < 0.6. This means that the incineration process is
3.1 Declared Unit considered a waste treatment process and included in the cal
1 m2 of VELUX Commercial polycarbonate rooflight is declared. culations. The generated 'exported energy' is assumed to have
reached the end­of­waste status and is considered in module
Declared unit and mass reference
D.
Name Value Unit
Declared unit 1 m2 Module A4 is not declared for being optional. In building
Grammage 36.9 kg/m2 assessments, the specific transport distance from
Kongerslev/Denmark to the construction site can be
A representative vaulted polycarbonate rooflight of the size
considered.
1200 mm x 2400 mm and with a hight of 300 mm is declared. It
consists of a 20 mm layer of polycarbonate and includes a
The products are delivered to the construction site ready to be
upstand of insulated wood (48 mm).
installed. Minor impacts from installation, e.g. using cranes, etc.
can be considered insignificant in the light of the total
3.2 System boundary
environmental impacts across the life cycle.
Type of the EPD: "cradle to gate with modules C1–C4, and
No packaging is used for the transport to the construction site
module D".
that would need to be disposed of in module A5. Module A5 is
not declared for being optional.
The production of VELUX Commercial polycarbonate rooflights
(modules A1-A3) includes raw material extraction, energy
Minor impacts from de­installation, e.g. using cranes, etc. can
generation, waste treatment and all transports up to the factory
be considered insignificant in the light of the total environmental
gate. In accordance with COUNCIL REGULATION (EU) No
impacts across the life cycle. The values of module C1 are
333/2011, secondary metals are modelled as part of the
hence 'zero'.
product system from the moment they are available as unmixed
scrap.
In the end­of­life, it is assumed that the disassembled products
For production wastes that are incinerated, it is as­sumed that
are brought to a sorting plant for construction materials, where
they are incinerated in a municipal waste incineration plant with
3 Environmental Product Declaration ­ VELUX Group ­ VELUX Commercial Polycarbonate rooflights (PC­ovenlys)
metals and burnable wastes are separeted. database.
Metals a are recycled; it is assumed that these fractions reach 3.6 Data quality
end­of­waste state after having been sorted and transported to The foreground data are based on extensive and detailed data
a recycler. Wooden parts and plastics are incinerated (also due collection at the production site. The foreground data could be
to the very limited data availability on plastics recycling and its fully linked with corresponding data records from the
benefits). On average, an average transport distance of 50 km background database ecoinvent v3.9.1 with the system model
has been assumed in module C2 with an average lorry for the "allocation – cut­off by classification – unit processes".
transport of the wastes to an incineration plant or to a recycling
facility. The background data was updated in 2022. Thus, the quality of
the foreground and background data can be rated as very
The disassembled product is shredded and the materials are good.
sorted in module C3. The recovered material leaves the The variability of the products consists only in its configuration
product system as 'materials for recycling'. The net amounts of (size). An estimate of the variance of results depending on the
the metals leaving the product system are considered as 'use of size of the products can be found in chapter 7.
secondary material' in Module D.
3.7 Period under review
The wooden parts and the plastics are treated in a waste
incineration plant with an efficiency R1 < 0.6 (according to The LCA data represents the production conditions for the year
CEWEP Energy Report III); the recovered energy is reported as 2022.
'exported energy' and considered in Module D.
3.8 Geographic Representativeness
Land or region, in which the declared product system is
Module C4 is not declared as a "recovery scenario" is assumed
manufactured, used or handled at the end of the product´s
on product level, including waste treatment from
lifespan: Europe
sorting/recycling in module C3.
Module D contains the benefits and loads beyond the system 3.9 Allocation
boundary related to the recycling of metals, which result from
No co­products are generated during the production of the
the treatment of recycled materials from the point of end­of­
VELUX Commercial products. Sorted production scrap of the
waste status to the point of substitution (as loads) and the
different metals, notably aluminium, is considered a secondary
substitution of primary resources (as benefits).
material with no economic value (so no burdens allocated) and
It also includes the benefits and loads related to the energy
considered in the quantification of net flows leaving the product
recovery from plastic and wooden wastes in a municipal waste
system. This approach is chosen to ensure a coherent
incineration plant as modelled in Module C3. Only net flows
quantification of net flows entering module D.
leaving the product system are considered in module D. The
recycled content and the assumed processing losses (e.g.,
Biogenic carbon is allocated based on physical flows
during remelting) are taken from ecoinvent v.3.9.1 datasets.
regardless of the allocation procedure chosen for the process.
The biogenic carbon content of wood products entering or
3.3 Estimates and assumptions
leaving the product system is quantified (manually) as part of
No further assumptions and estimates relevant to the result had
the GWP in conformity with EN 16485.
to be made beyond the points made in chapter 3 and chapter 4.
3.4 Cut-off criteria No processes were modelled as part of the foreground model
that would have required an allocation of multi­input processes.
No data available from the company survey was neglected.
Background datasets on municipal waste incineration plants
These include, among other things, material use, energy
were taken from ecoinvent without any modification.
demand (heat, electricity), packaging materials of raw materials
(insofar as they are generated as waste) and product
Allocation of reuse, recycling and recovery was avoided by the
packaging, consumables in production, waste treatment and
cut­off approach in the foreground model in line with EN 15804.
the transport of all inputs and outputs.
With this approach, mass and energy flows below 1 % were
3.10 Comparability
also accounted for. No processes were neglected that would
Basically, a comparison or an evaluation of EPD data is only
have been known to the project managers and would have
possible if all the data sets to be compared were created
contributed significantly to the indicators of the impact
according to EN 15804 and the building context, respectively
assessment.
the product­specific characteristics of performance, are taken
into account.
3.5 Background data Ecoinvent v3.9.1 (2022) with the system model 'allocation – cut­
off by classification – unit processes' is used as the background
Ecoinvent v3.9.1 (2022) with the system model 'allocation – cut­
database.
off by classification – unit processes' is used as the background
4. LCA: Scenarios and additional technical information
Name ValueUnit
Characteristic product properties of biogenic carbon
kg
Biogenic carbon content in product ­
Information on describing the biogenic carbon content at C
factory gate Biogenic carbon content in accompanying kg
9.85
Note: 1 kg of biogenic carbon is equivalent to 44/12 kg of CO 2. packaging C
Reference service life
4 Environmental Product Declaration ­ VELUX Group ­ VELUX Commercial Polycarbonate rooflights (PC­ovenlys)
Name Value Unit Module C1
Inputs and outputs from de­installation are disregared.
Life Span according to the
30 a
manufacturer
Module C2
The product has passed
Declared product On average, an transport distance of 50 km to a
internal quality controls and
properties (at the gate) and ­ sorting/recycling facility and an additional 50 km for sorted
complies with product
finishes wooden and plastic parts to a municipal waste incineration
standard for CE marking
plant.
Design application
parameters (if instructed by
Installation according to Module C3
the manufacturer),
assembly instructions and ­ A consumption of 0.03 kWh/kg of electricity for shredding and
including the references to
state of the art. sorting and 0.437 MJ/kg of diesel fuel for internal logistics are
the appropriate practices
taken into account to disassemble the product. The recovered
and application codes
material leaves the product system as 'materials for recycling'.
An assumed quality of The net amounts of the metals leaving the product system are
Carried out in accordance
work, when installed in considered as 'use of secondary material' in Module D.
with the manufacturer's ­
accordance with the
instructions.
manufacturer’s instructions As stated above, it is assumed that 100 % of the wooden and
Outdoor environment, (for The declared products are plastic parts are treated in a waste incineration plant with an
outdoor applications), e.g. intended for installation efficiency R1 < 0.6 (according to CEWEP Energy Report III);
weathering, pollutants, UV outside the building: They are according to the same source, an efficiency of 31.0 % is
­
and wind exposure, therefore designed to assumed for the production of heat and 18.0 % for the
building orientation, withstand outdoor conditions production of electricity (always referring to the lower heating
shading, temperature throughout their service life. value of the waste). The recovered energy is reported as
Indoor environment (for 'exported energy' and considered in Module D.
The declared products are
indoor applications), e.g.
temperature, moisture, not intended for installation ­ Module C4
chemical exposure inside a building. Not relevant according to the assumed end­of­life scenario.
Usage conditions, e.g. Standard use in any type of
Module D
frequency of use, building, i.e., opening/closing ­
Module D contains the benefits and loads beyond the system
mechanical exposure as often as necessary.
boundary related to the recycling of metals, which result from
The declared products are
the treatment of recycled materials from the point of end­of­
Maintenance e.g. required designed for a reference
waste status to the point of substitution (as loads) and the
frequency, type and quality service life of 30 years. They
­ substitution of primary resources (as benefits).
and replacement of are maintained by cleaning
It also includes the benefits and loads related to the energy
components water at the discretion of the
recovery from wooden and plastic wastes in a municipal waste
building occupants.
incineration plant as modelled in Module C3.
Only net flows leaving the product system are considered in
module D.
5 Environmental Product Declaration ­ VELUX Group ­ VELUX Commercial Polycarbonate rooflights (PC­ovenlys)
5. LCA: Results
The set of characterisation factors EF 3.1 has been used.
DESCRIPTION OF THE SYSTEM BOUNDARY (X = INCLUDED IN LCA; MND = MODULE OR INDICATOR NOT DECLARED; MNR
= MODULE NOT RELEVANT)
Benefits and
Construction loads beyond
Product stage Use stage End of life stage
process stage the system
boundaries
la ire ta m w a Ry lp p u s tro p s n a rT g n iru tc a fu n a M e h t m o rf tro p s n a rTe tis e h t o t e ta g y lb m e s s A e s U e c n a n e tn ia M ria p e R tn e m e c a lp e R tn e m h s ib ru fe R y g re n e la n o ita re p Oe s u re ta w la n o ita re p Oe s u n o itc u rts n o c ­e Dn o itilo m e d tro p s n a rT g n is s e c o rp e ts a W la s o p s iD ­e s u e R­y re v o c e R­g n ilc y c e Rla itn e to p
A1 A2 A3 A4 A5 B1 B2 B3 B4 B5 B6 B7 C1 C2 C3 C4 D
X X X MND MND MND MND MNR MNR MNR MND MND X X X X X
RESULTS OF THE LCA - ENVIRONMENTAL IMPACT according to EN 15804+A2: 1 m² of VELUX Commercial polycarbonate
rooflights
Parameter Unit A1-A3 C1 C2 C3 C4 D
Global Warming Potential total (GWP­total) kg CO 2 eq 8.69E+01 0 5.1E­01 5.42E+01 0 ­1.24E+02
Global Warming Potential fossil fuels (GWP­fossil) kg CO 2 eq 1.2E+02 0 5.09E­01 2.09E+01 0 ­1.18E+02
Global Warming Potential biogenic (GWP­biogenic) kg CO 2 eq ­3.36E+01 0 4.27E­04 3.33E+01 0 ­5.65E+00
Global Warming Potential luluc (GWP­luluc) kg CO 2 eq 2.62E­01 0 2.49E­04 1.57E­03 0 ­2.77E­01
Depletion potential of the stratospheric ozone layer (ODP) kg CFC11 eq 4.17E­06 0 1.12E­08 1.72E­07 0 ­1.62E­06
Acidification potential of land and water (AP) mol H+ eq 7.22E­01 0 2.38E­03 2.77E­02 0 ­4.51E­01
Eutrophication potential aquatic freshwater (EP­freshwater) kg P eq 4.68E­03 0 4.18E­06 1.03E­04 0 ­1.04E­02
Eutrophication potential aquatic marine (EP­marine) kg N eq 1.31E­01 0 9.37E­04 1.23E­02 0 ­7.41E­02
Eutrophication potential terrestrial (EP­terrestrial) mol N eq 1.53E+00 0 1.01E­02 1.36E­01 0 ­8.51E­01
Formation potential of tropospheric ozone photochemical oxidants kg NMVOC
5.79E­01 0 3.53E­03 3.83E­02 0 ­2.71E­01
(POCP) eq
Abiotic depletion potential for non fossil resources (ADPE) kg Sb eq 7.07E­04 0 1.59E­06 4.25E­06 0 1.13E­04
Abiotic depletion potential for fossil resources (ADPF) MJ 1.8E+03 0 7.35E+00 3.55E+01 0 ­1.49E+03
m3 world eq
Water use (WDP) 4.08E+01 0 3.2E­02 3.87E­01 0 ­8.84E+00
deprived
RESULTS OF THE LCA - INDICATORS TO DESCRIBE RESOURCE USE according to EN 15804+A2: 1 m² of VELUX Commercial
polycarbonate rooflights
Parameter Unit A1-A3 C1 C2 C3 C4 D
Renewable primary energy as energy carrier (PERE) MJ 4.68E+02 0 1.15E­01 3.97E+02 0 ­2.28E+02
Renewable primary energy resources as material utilization
MJ 3.95E+02 0 0 ­3.95E+02 0 0
(PERM)
Total use of renewable primary energy resources (PERT) MJ 8.63E+02 0 1.15E­01 2.19E+00 0 ­2.28E+02
Non renewable primary energy as energy carrier (PENRE) MJ 1.56E+03 0 7.35E+00 2.77E+02 0 ­1.51E+03
Non renewable primary energy as material utilization (PENRM) MJ 2.41E+02 0 0 ­2.41E+02 0 0
Total use of non renewable primary energy resources (PENRT) MJ 1.81E+03 0 7.35E+00 3.57E+01 0 ­1.51E+03
Use of secondary material (SM) kg 1.31E+00 0 0 0 0 3.16E+00
Use of renewable secondary fuels (RSF) MJ 0 0 0 0 0 0
Use of non renewable secondary fuels (NRSF) MJ 0 0 0 0 0 0
Use of net fresh water (FW) m3 2.65E+00 0 1.99E­03 3.63E­02 0 ­6.83E­01
RESULTS OF THE LCA – WASTE CATEGORIES AND OUTPUT FLOWS according to EN 15804+A2:
1 m² of VELUX Commercial polycarbonate rooflights
Parameter Unit A1-A3 C1 C2 C3 C4 D
Hazardous waste disposed (HWD) kg 1.48E­02 0 4.63E­05 1.85E­04 0 4.22E­03
Non hazardous waste disposed (NHWD) kg 2.7E+01 0 4.68E­01 3.17E+00 0 ­1.58E+01
Radioactive waste disposed (RWD) kg 4.58E­03 0 4.31E­06 8.77E­05 0 ­7.51E­03
Components for re­use (CRU) kg 0 0 0 0 0 0
Materials for recycling (MFR) kg 1.7E­01 0 0 4.3E+00 0 4.3E+00
Materials for energy recovery (MER) kg 0 0 0 0 0 0
Exported electrical energy (EEE) MJ 5.45E+00 0 0 1.14E+02 0 0
Exported thermal energy (EET) MJ 9.39E+00 0 0 1.97E+02 0 0
RESULTS OF THE LCA – additional impact categories according to EN 15804+A2-optional:
1 m² of VELUX Commercial polycarbonate rooflights
Parameter Unit A1-A3 C1 C2 C3 C4 D
Disease
Incidence of disease due to PM emissions (PM) 9.41E­06 0 5E­08 5.09E­07 0 ­4.68E­06
incidence
Human exposure efficiency relative to U235 (IR) kBq U235 eq 3.18E+00 0 3.81E­03 4.8E­02 0 ­3.39E+00
6 Environmental Product Declaration ­ VELUX Group ­ VELUX Commercial Polycarbonate rooflights (PC­ovenlys)
Comparative toxic unit for ecosystems (ETP­fw) CTUe 1.93E+03 0 3.62E+00 7.44E+01 0 ­3.16E+02
Comparative toxic unit for humans (carcinogenic) (HTP­c) CTUh 2.22E­07 0 2.74E­10 1.01E­08 0 ­6.53E­08
Comparative toxic unit for humans (noncarcinogenic) (HTP­nc) CTUh 1.95E­06 0 5.7E­09 4.23E­08 0 ­8.35E­07
Soil quality index (SQP) SQP 4.39E+03 0 5.53E+00 5.09E+00 0 ­1.99E+02
Disclaimer 1 – for the indicator “Potential Human exposure efficiency relative to U235”. This impact category deals mainly with the
eventual impact of low­dose ionizing radiation on human health of the nuclear fuel cycle. It does not consider effects due to possible
nuclear accidents, occupational exposure or radioactive waste disposal in underground facilities. Potential ionizing radiation from the
soil, radon and from some construction materials is also not measured by this indicator.
Disclaimer 2 – for the indicators “abiotic depletion potential for non­fossil resources”, “abiotic depletion potential for fossil resources”,
“water (user) deprivation potential, deprivation­weighted water consumption”, “potential comparative toxic unit for ecosystems”,
“potential comparative toxic unit for humans – cancerogenic”, “Potential comparative toxic unit for humans ­ not cancerogenic”,
“potential soil quality index”. The results of this environmental impact indicator shall be used with care as the uncertainties on these
results are high as there is limited experience with the indicator.
6. LCA: Interpretation
Figure 1 illustrates the relative contributions of the different polycarbonate rooflights.
modules along the life cycle for VELUX Commercial
product life cycle, except for the ADPelements (modules A1­
Figure 1: Relative environmental impacts of the different C4). The net positive impact ('load') of the ADPelements is
life cycle stages for VELUX Commercial polycarbonate related to copper input as the copper cathode for the remelting
rooflights (modules A1–A3 = 100 %) of recycled aluminium.
By far the largest part of environmental impacts is caused The use of renewable primary energy is caused on the one
during production (modules A1­A3) of the VELUX Commercial hand by the share of renewable energy in the electricity mix
polycarbonate rooflights. The contributions of other life cycle and on the other hand by the primary energy content of sawn
stages are comparably small. timber and plywood used in the upstand; the production stage
is the main driver of this impact category whereas the
Benefits and burdens beyond the system boundary (module D) renewable energy stored in the wooden material is rebooked as
are in the order of ­216 % to ­21 % of the impacts over the used as an energy carrier in module C3.
7 Environmental Product Declaration ­ VELUX Group ­ VELUX Commercial Polycarbonate rooflights (PC­ovenlys)
use phase.
The use of non­renewable primary energy is mainly caused on
the one hand by the share of non­renewable energy in the
electricity mix and heat consumption during production and on The LCA for the VELUX Commercial products have been
the other hand by the primary energy content of the plastic calculated for representative products, which are in fact quite
materials (polycarbonate and acrylic); the production stage is close to the composition of the weighted average production in
the main driver of this impact category whereas the non­ 2022. To assess the possible variance, a 'maximum' version in
renewable energy stored in the plastic components is rebooked terms of material intensity (highest upstand, highest number of
as used as an energy carrier in module C3. acrylic/polycarbonate layers, etc.) has been assessed per
product group. The higher material intensity of the maximum
Non­hazardous waste as the quantitatively most relevant waste version is more than compensated by a higher surface area
flows is mainly caused during maintenance due to the covered but lead to lower impact of around 10 % in most impact
replacement of the motor; hazardous and radioactive waste are indicators.
mainly caused by the European electricity mix used during the
7. Requisite evidence
7.1 Formaldehyde Not applicable; no test defined in applicable product standards.
No test defined in applicable product standards.
7.4 Fire gas toxicity
7.2 MDI No test defined in applicable product standards.
No test defined in applicable product standards.
7.5 VOC emissions
7.3 Checking for pretreatment of the substances used No test defined in applicable product standards.
(Measurement according to AltholzV)
8. References
Product category rules of IBU DIN EN ISO 14025:2006­07, Environmental labels and
declarations ­ Type III Environmental declarations ­ Principles
IBU (2021) and procedures.
IBU (2021): General Instructions for the EPD Programme of the
Institut Bauen und Umwelt e.V. Version 2.0, Institut Bauen und ISO 14044
Umwelt, Berlin. DIN EN ISO 14044:2006­07, Environmental management ­ Life
cycle assessment ­ Requirements and guidance.
IBU (2021)
IBU (2021): PCR Part A: Calculation rules for the life cycle ECHA candidate list
assessment and requirements on the project report according The candidate list of substances of very high concern,
to EN 15804+A2. Version 1.3, Institut Bauen und Umwelt e.V., European Chemicals Agency, Helsinki. Available at:
Berlin. https://echa.europa.eu/nl/­/four­newsubstances­added­to­the
candidate­list.
IBU (2023)
IBU (2023): PCR Part B: Requirements on the EPD for Regulation on biocidal products
windows and doors. Version 2023/04, Institut Bauen und REGULATION (EU) No 528/2012 OF THE EUROPEAN
Umwelt e.V., Berlin. PARLIAMENT AND OF THE COUNCIL of 22 May 2012
concerning the making available on the market and use of
Standards and legal documents biocidal products.
EN 1873 Regulation (EU) Nr. 305/2011(CPR)
DIN EN 1873:2005, Prefabricated accessories for roofing ­ REGULATION (EU) No 305/2011 OF THE EUROPEAN
Individual rooflights of plastics ­ Product specification and test PARLIAMENT AND OF THE COUNCIL of 9 March 2011 laying
methods. down harmonised conditions for the marketing of construction
products and repealing Council Directive 89/106/EEC.
EN 15804
DIN EN 15804+A2:2022­03, sustainability of construction COUNCIL REGULATION (EU) No 333/2011
works ­ Environmental product declarations ­ Core rules for the COUNCIL REGULATION (EU) No 333/2011 of 31 March 2011
product category construction products; German version EN establishing criteria determining when certain types of scrap
15804: 2012+A2:2019 + AC:2021. metal cease to be waste under Directive 2008/98/EC of the
European Parliament and of the Council.
EN 16485
DIN EN 16485:2014­07, Round and sawn timber ­ European Waste List (Waste index)
Environmental Product Declarations ­ Product category rules http://www.gesetze­im­internet.de/avv/anlage.htm
for wood and wood­based products for use in construction;
German version EN 16485:2014. Additional references
ISO 9001 CEWEP Energy Report III
DIN EN ISO 9001:2015, Quality management systems ­ Reimann D.O. (2013): CEWEP Energy Report III (Status 2007
Requirements. – 2010); Results of Specific Data for Energy, R1 Plant
Efficiency Factor and NCV of 314 European Waste­to­Energy
ISO 14025 (WtE) Plants. CEWEP, Würzburg/Brussels, 2013.
8 Environmental Product Declaration ­ VELUX Group ­ VELUX Commercial Polycarbonate rooflights (PC­ovenlys)
ecoinvent v3.9.1, LCA database, 12/2022. Ecoinvent centre,
ecoinvent v3.9.1 Zürich.
9 Environmental Product Declaration ­ VELUX Group ­ VELUX Commercial Polycarbonate rooflights (PC­ovenlys)
Publisher
Institut Bauen und Umwelt e.V. +49 (0)30 3087748­ 0
Hegelplatz 1 info@ibu­epd.com
10117 Berlin www.ibu­epd.com
Germany
Programme holder
Institut Bauen und Umwelt e.V. +49 (0)30 3087748­ 0
Hegelplatz 1 info@ibu­epd.com
10117 Berlin www.ibu­epd.com
Germany
Author of the Life Cycle Assessment
Dr. Frank Werner ­ Umwelt & Entwicklung + 41 (0)44 241 39 06
Kammelenbergstrasse 30 frank@frankwerner.ch
9011 St. Gallen http://www.frankwerner.ch/
Switzerland
Owner of the Declaration
VELUX Group +4545164871
Ådalsvej 99 birthe.kjeldsen@velux.com
2970 Hørsholm www.velux.com
Denmark
10 Environmental Product Declaration ­ VELUX Group ­ VELUX Commercial Polycarbonate rooflights (PC­ovenlys)
