ENVIRONMENTAL PRODUCT DECLARATION
as per ISO 14025 and EN 15804+A2
Owner of the Declaration Sto SE & Co. KGaA
Publisher Institut Bauen und Umwelt e.V. (IBU)
Programme holder Institut Bauen und Umwelt e.V. (IBU)
Declaration number EPD-STO-20230193-IBA1-EN
Issue date 11.08.2023
Valid to 10.08.2028
StoVentec Carrier Board S
Sto SE & Co. KGaA
www.ibu-epd.com | https://epd-online.com
General Information
Sto SE & Co. KGaA StoVentec Carrier Board S
Programme holder Owner of the declaration
IBU – Institut Bauen und Umwelt e.V. Sto SE & Co. KGaA
Hegelplatz 1 Ehrenbachstr. 1
10117 Berlin 79780 Stühlingen
Germany Germany
Declaration number Declared product / declared unit
EPD-STO-20230193-IBA1-EN 1 m² carrier board (12 mm) with formulation in the quality (class) A2-s1, d0
in accordance with EN 13501-1 (name: StoVentec Carrier Board S).
This declaration is based on the product category rules: Scope:
Lightweight boards made of lightweight fillers and reactive resins, This EPD relates to carrier boards made of lightweight filler material
01.08.2021 (expanded glass or perlite granulate) and reactive resins with formulations
(PCR checked and approved by the SVR) in the qualities (classes) B1 in accordance with DIN 4102-1 and A2-s1, d0
in accordance with EN 13501-1. These are produced by Verotec GmbH,
Hanns-Martin-Schleyer-Straße 1, 89415 Lauingen, Germany. This is an
Issue date environmental product declaration for a specific product named StoVentec
Carrier Board S (made of expanded glass granulate) in the quality (class)
11.08.2023
A2-s1,d0 in accordance with EN 13501-1, while the following board types
(formulations) and their environmental effects are described in the annex.
Formulation in quality (class) A2-s1,d0 in accordance with EN 13501-1 -
Valid to
made of expanded glass granulate:
10.08.2028
• StoVentec Carrier Board A (12 mm)
• StoPanel Plus (12 mm)
• StoPanel Plus (20 mm)
• StoPrefa Render Carrier Board (12 mm)
Formulation in quality (class) B1 in accordance with DIN 4102-1 - made of
expanded glass granulate:
• StoVentec Carrier Board (12 mm)
• Sto-Render Carrier Board (20 mm)
• StoPrefa Shutter Board (20 mm)
Formulation in quality (class) A2-s1,d0 in accordance with EN 13501-1 -
made of expanded perlite granulate:
Dipl.-Ing. Hans Peters • Verolith Carrier Board (15 mm)
(Chairman of Institut Bauen und Umwelt e.V.) The owner of the declaration shall be liable for the underlying information
and evidence; the IBU shall not be liable with respect to manufacturer
information, life cycle assessment data and evidences.
The EPD was created according to the specifications of EN 15804+A2. In
the following, the standard will be simplified as EN 15804.
Verification
The standard EN 15804 serves as the core PCR
Independent verification of the declaration and data according to ISO
14025:2011
internally X externally
Florian Pronold Matthias Schulz,
(Managing Director Institut Bauen und Umwelt e.V.) (Independent verifier)
1 Environmental Product Declaration - Sto SE & Co. KGaA - StoVentec Carrier Board S
Product
Other constructional data are not relevant.
Product description/Product definition
Pressed carrier boards made of lightweight fillers (expanded Product performance values in relation to its characteristics
glass or perlite granulate) and reactive resins with glass fibre according to the relevant technical regulations (no CE marking).
mesh reinforcement on both sides. The expanded glass
granulate is made of recycled glass while the perlite granulate Base materials/Ancillary materials
is a natural material of volcanic origin. The declared product is Name Value Unit
named "StoVentec Carrier Board S" and is based on expanded Expanded glass granulate < 85 Mass [%]
glass granulate with reactive resins in the quality (class) A2-
Filling materials < 20 Mass [%]
s1,d0 in accordance with EN 13501-1.
Propellant and hydrophobic agents < 1 Mass [%]
The following technical data and calculations refer to the
declared product. Reactive polymer resin < 10 Mass [%]
Hardener < 2 Mass [%]
Placing on the market/appliaction rules Glass fibre mesh < 7 Mass [%]
The relevant national regulations at the site of use apply when
using this product. In Germany, for example, these are the
building regulations that apply within the individual federal
1. This products contains substances listed in the
states and the technical provisions based on these regulations.
candidate list (17 January 2023) exceeding 0.1
For the use and application of the product the respective
percentage by mass: no
national provisions at the place of use apply, in Germany for
2. This product contains other CMR substances in
example the building codes of the federal states and the
categories 1A or 1B which are not on the candidate list,
corresponding national specifications.
exceeding 0.1 percentage by mass: no
Application 3. Biocide products were added to this construction
The carrier boards are suitable for use in rainscreen cladding product or it has been treated with biocide products (this
systems or for ceiling claddings in outdoor areas. They can also then concerns a treated product as defined by the (EU)
be used in combination with external wall insulation systems Ordinance on Biocide Products No. 528/2012: no
and in interiors. 4. This product contains fire retardants: yes / aluminium
hydroxide
Technical Data
Reference service life
Constructional data
According to the Bewertungssystem Nachhaltiges Bauen (BNB)
Name Value Unit Sustainable Building assessment system of 7 July 2011, the
Gross density TIAP 120 (Sto internal) ca. 500 kg/m3 carrier board approximately corresponds to Code Nr. 335.915
(BNB), wall coverings (systems): plastic, multi-layer lightweight
Thermal conductivity DIN 52612 0.12 W/(mK)
construction boards with a service life of 40 years. The board
1800 –
Modulus of elasticity EN ISO 178 N/mm² structure of recycled glass and reactive resin is extremely
2000
stable in its coated state. The reference service life could
Thermal expansion TIAP 650 (Sto-intern) 0,000011 1/K
therefore be synonymous with the service life of the
Water vapour diffusion-equivalent air layer structure/building element.
15 µ
thickness EN ISO 7783-2
LCA: Calculation rules
· A2 Transport of raw materials to the manufacturer,
Declared Unit · A3 Production of StoVentec Carrier Board S in the factory,
The declaration refers to 1m² StoVentec Carrier Board S of (incl. energy provision, water provision, disposal of production
thickness 12mm. waste, production of packaging materials)
Declared unit
Construction stage (A4-A5): The construction
Name Value Unit
process stage includes:
Declared unit 1 m2 · A4 transport to the construction site 100km by
Gross density 535 kg/m3 truck,
Grammage 6.42 kg/m2 · A5 installation of the product with machine and treatment of
the packaging materials in waste incineration units after
Layer thickness 0.012 m
installation of the
product
End-of-life stage (C1-C4): The end-of-life stage
System boundary
includes:
Type of EPD: Cradle to gate with options, modules C1-C4 and · C1 de-construction with machine
module D (A1-A3 + C + D and additional modules: A4, A5). The · C2 transport to waste processing; 50 km with truck
LCA considers the following modules of the life cycle: Transport distance can be adjusted at building level if
necessary (e.g., for 100 km actual transport distance:
Production Stage (A1-A3): The Product stage multiply LCA values by factor 2).
includes: · C4 disposal of
· A1 Raw material supply and processing, the product in a landfill for inert matter
2 Environmental Product Declaration - Sto SE & Co. KGaA - StoVentec Carrier Board S
Benefits and loads beyond the Comparability
System Boundary (D): Module D includes: Basically, a comparison or an evaluation of EPD data is only
Energy recovery potentialsfrom the thermal treatment of the possible if all the data sets to be compared were created
pallets, paper and plastic waste from packaging according to EN 15804 and the building context, respectively
the product-specific characteristics of performance, are taken
Geographic Representativeness into account. The background data comes from the GaBi
Land or region, in which the declared product system is database GaBi software Version CUP2022.2
manufactured, used or handled at the end of the product´s
lifespan: Europe
LCA: Scenarios and additional technical information
Name Value Unit
Characteristic product properties of biogenic carbon
wooden pallets 0.047 kg
Paper 0.018 kg
Information on describing the biogenic Carbon Content at
polyethylene 0.002 kg
factory gate
Diesel consumption 0.01 l/10 kg
Name ValueUnit
kg
Biogenic carbon content in product -
C End of the life cycle (C1-C4)
Biogenic carbon content in accompanying kg
0.026
packaging C Deconstruction (C1)
The product dismantling from the building is done with a
machine
Transport to EoL treatment (C2)
Transportfrom the gate to the site (A4) Transport to waste treatment: 50 km by truck
Name Value Unit
Transport distance 100 km Disposal (C4)
landfilling (EU)
Installation into the building (A5) Name Value Unit
Module A5 includes the installation of the product with a Landfilling 6.42 kg
machine and the treatment and disposal of packaging material.
Benefits for potential avoided burdens due to energy Reuse, recovery and/or recycling potentials (D), relevant
substitution of electricity and thermal energy generation are scenario information
declared in module D and affect only the rate of primary Name Value Unit
material (no secondary materials)
For energy recovery (packaging) 0.049 kg
No credit for paper has been taken as waste paper has been
used.
3 Environmental Product Declaration - Sto SE & Co. KGaA - StoVentec Carrier Board S
LCA: Results
DESCRIPTION OF THE SYSTEM BOUNDARY (X = INCLUDED IN LCA; ND = MODULE OR INDICATOR NOT DECLARED; MNR =
MODULE NOT RELEVANT)
Benefits and
Construction loads beyond
Product stage Use stage End of life stage
process stage the system
boundaries
la ire ta m w a Ry lp p u s tro p s n a rT g n iru tc a fu n a M e h t m o rf tro p s n a rTe tis e h t o t e ta g y lb m e s s A e s U e c n a n e tn ia M ria p e R tn e m e c a lp e R tn e m h s ib ru fe R y g re n e la n o ita re p Oe s u re ta w la n o ita re p Oe s u n o itc u rts n o c -e Dn o itilo m e d tro p s n a rT g n is s e c o rp e ts a W la s o p s iD -e s u e R-y re v o c e R-g n ilc y c e Rla itn e to p
A1 A2 A3 A4 A5 B1 B2 B3 B4 B5 B6 B7 C1 C2 C3 C4 D
X X X X X MND MND MNR MNR MNR MND MND X X X X X
RESULTS OF THE LCA - ENVIRONMENTAL IMPACT according to EN 15804+A2: 1 m² StoVentec Carrier Board S (12mm)
Parameter Unit A1-A3 A4 A5 C1 C2 C3 C4 D
GWP-total kg CO 2 eq 9.36E+00 4.18E-02 1.24E-01 3.31E-02 2.09E-02 0 9.77E-02 -2.96E-02
GWP-fossil kg CO 2 eq 9.34E+00 4.18E-02 3.76E-02 3.16E-02 2.09E-02 0 9.74E-02 -2.95E-02
GWP-biogenic kg CO 2 eq 1.89E-02 0 8.64E-02 1.48E-03 0 0 0 -1.51E-04
GWP-luluc kg CO 2 eq 1.57E-03 6.81E-07 7.43E-07 5.23E-07 3.4E-07 0 2.8E-04 -3.24E-06
ODP kg CFC11 eq 3.45E-11 6.35E-15 1.22E-14 4.88E-15 3.17E-15 0 3.61E-16 -2E-13
AP mol H+ eq 2.11E-02 3.18E-05 1.86E-04 1.74E-04 1.59E-05 0 6.99E-04 -3.88E-05
EP-freshwater kg P eq 2.11E-05 8.68E-09 8.43E-09 6.67E-09 4.34E-09 0 1.67E-07 -4.06E-08
EP-marine kg N eq 6.64E-03 1.06E-05 9.08E-05 8.67E-05 5.31E-06 0 1.8E-04 -1.05E-05
EP-terrestrial mol N eq 7.65E-02 1.18E-04 1.01E-03 9.49E-04 5.91E-05 0 1.98E-03 -1.13E-04
kg NMVOC
POCP 1.83E-02 3.01E-05 2.43E-04 2.32E-04 1.51E-05 0 5.45E-04 -2.95E-05
eq
ADPE kg Sb eq 2.5E-06 2.33E-09 1.97E-09 1.79E-09 1.16E-09 0 8.74E-09 -4.45E-09
ADPF MJ 1.45E+02 5.86E-01 4.7E-01 4.5E-01 2.93E-01 0 1.28E+00 -5.02E-01
m3 world eq
WDP 1.28E-01 4.8E-05 9.38E-03 3.69E-05 2.4E-05 0 1.02E-02 -3.14E-03
deprived
GWP = Global warming potential; ODP = Depletion potential of the stratospheric ozone layer; AP = Acidification potential of land and water; EP =
Eutrophication potential; POCP = Formation potential of tropospheric ozone photochemical oxidants; ADPE = Abiotic depletion potential for non-fossil
resources; ADPF = Abiotic depletion potential for fossil resources; WDP = Water (user) deprivation potential)
RESULTS OF THE LCA - INDICATORS TO DESCRIBE RESOURCE USE according to EN 15804+A2: 1 m² StoVentec Carrier
Board S (12mm)
Parameter Unit A1-A3 A4 A5 C1 C2 C3 C4 D
PERE MJ 1.62E+01 3.4E-03 1.03E+00 2.61E-03 1.7E-03 0 1.67E-01 -1.38E-01
PERM MJ 1.02E+00 0 -1.02E+00 0 0 0 0 0
PERT MJ 1.73E+01 3.4E-03 7.19E-03 2.61E-03 1.7E-03 0 1.67E-01 -1.38E-01
PENRE MJ 1.25E+02 5.86E-01 5.58E-01 4.51E-01 2.93E-01 0 2.11E+01 -5.02E-01
PENRM MJ 1.99E+01 0 -8.83E-02 0 0 0 -1.98E+01 0
PENRT MJ 1.45E+02 5.86E-01 4.7E-01 4.51E-01 2.93E-01 0 1.28E+00 -5.02E-01
SM kg 0 0 0 0 0 0 0 0
RSF MJ 0 0 0 0 0 0 0 0
NRSF MJ 0 0 0 0 0 0 0 0
FW m3 2.13E-02 2.89E-06 2.22E-04 2.22E-06 1.44E-06 0 3.22E-04 -1.33E-04
PERE = Use of renewable primary energy excluding renewable primary energy resources used as raw materials; PERM = Use of renewable primary
energy resources used as raw materials; PERT = Total use of renewable primary energy resources; PENRE = Use of non-renewable primary energy
excluding non-renewable primary energy resources used as raw materials; PENRM = Use of non-renewable primary energy resources used as raw
materials; PENRT = Total use of non-renewable primary energy resources; SM = Use of secondary material; RSF = Use of renewable secondary fuels;
NRSF = Use of non-renewable secondary fuels; FW = Use of net fresh water
RESULTS OF THE LCA – WASTE CATEGORIES AND OUTPUT FLOWS according to EN 15804+A2:
1 m² StoVentec Carrier Board S (12mm)
Parameter Unit A1-A3 A4 A5 C1 C2 C3 C4 D
HWD kg 2.21E-08 1.96E-12 3.37E-12 1.5E-12 9.78E-13 0 1.95E-08 -6.79E-11
NHWD kg 7.95E-01 7.06E-05 1.1E-03 5.42E-05 3.53E-05 0 6.43E+00 -2.54E-04
RWD kg 3.47E-03 5.21E-07 1.52E-06 4E-07 2.6E-07 0 1.45E-05 -3.95E-05
CRU kg 0 0 0 0 0 0 0 0
MFR kg 0 0 0 0 0 0 0 0
MER kg 0 0 0 0 0 0 0 0
EEE MJ 0 0 1.33E-01 0 0 0 0 0
EET MJ 0 0 2.38E-01 0 0 0 0 0
4 Environmental Product Declaration - Sto SE & Co. KGaA - StoVentec Carrier Board S
HWD = Hazardous waste disposed; NHWD = Non-hazardous waste disposed; RWD = Radioactive waste disposed; CRU = Components for re-use;
MFR = Materials for recycling; MER = Materials for energy recovery; EEE = Exported electrical energy; EET = Exported thermal energy
RESULTS OF THE LCA – additional impact categories according to EN 15804+A2-optional:
1 m² StoVentec Carrier Board S (12mm)
Parameter Unit A1-A3 A4 A5 C1 C2 C3 C4 D
Disease
PM 1.8E-07 1.78E-10 3.64E-09 3.57E-09 8.88E-11 0 8.65E-09 -3.21E-10
incidence
IR kBq U235 eq 3.25E-01 4.66E-05 2.18E-04 3.59E-05 2.33E-05 0 1.49E-03 -6.69E-03
ETP-fw CTUe 1.33E+02 4.66E-01 3.67E-01 3.58E-01 2.33E-01 0 7.3E-01 -1.1E-01
HTP-c CTUh 2.82E-09 8.74E-12 7.32E-12 6.72E-12 4.37E-12 0 1.08E-10 -5.06E-12
HTP-nc CTUh 2.32E-07 3.76E-10 3.95E-10 3.69E-10 1.88E-10 0 1.19E-08 -1.96E-10
SQP SQP 2.55E+01 2.55E-03 7.67E-03 1.96E-03 1.27E-03 0 2.66E-01 -8.95E-02
PM = Potential incidence of disease due to PM emissions; IR = Potential Human exposure efficiency relative to U235; ETP-fw = Potential comparative
Toxic Unit for ecosystems; HTP-c = Potential comparative Toxic Unit for humans (cancerogenic); HTP-nc = Potential comparative Toxic Unit for humans
(not cancerogenic); SQP = Potential soil quality index
Disclaimer 1 – for the indicator “Potential Human exposure efficiency relative to U235”. This impact category deals mainly with the
eventual impact of low-dose ionizing radiation on human health of the nuclear fuel cycle. It does not consider effects due to possible
nuclear accidents, occupational exposure or radioactive waste disposal in underground facilities. Potential ionizing radiation from the
soil, radon and from some construction materials is also not measured by this indicator.
Disclaimer 2 – for the indicators “abiotic depletion potential for non-fossil resources”, “abiotic depletion potential for fossil resources”,
“water (user) deprivation potential, deprivation-weighted water consumption”, “potential comparative toxic unit for ecosystems”,
“potential comparative toxic unit for humans – cancerogenic”, “Potential comparative toxic unit for humans - not cancerogenic”,
“potential soil quality index”. The results of this environmental impact indicator shall be used with care as the uncertainties on these
results are high as there is limited experience with the indicator.
References
Standards 2: Determination and classification of water vapour
transmission rate (permeability) (ISO 7783-2:1999), 1999-06
DIN 18516-1
DIN 18516-1:2010-06 Cladding for external walls, ventilated at ISO 14025
rear – Part 1: Requirements, principles of testing EN ISO 14025:2011, Environmental labels and declarations —
Type III environmental declarations — Principles and
DIN 4102 procedures.
DIN 4102:1998 Fire behaviour of building materials and
building components – Part 1: Building materials; concepts, Further Refererences
requirements and tests
Committee for Health-related Evaluation of Building
DIN 52612 Products
DIN 52612:1984 Testing of thermal insulating materials; Committee for Health-related Evaluation of Building Products,
determination of thermal conductivity by means of the guarded 2010: assessment scheme for VOC from building products.
hot plate apparatus; conversion of the measured values for 2010
building applications
CML
DIN EN ISO 178 CML-IA Characterisation Factors; Institute of Environmental
DIN EN ISO 178:2010 Plastics – Determination of flexural Sciences, 5 February 2013: http://cml.leiden.edu/software/data-
properties (ISO 178:2010); German version EN ISO 178:2010, cmlia.html
2011-04
Code Nr. 335.915
DIN EN 13501-1 Code Nr. 335.915 (BNB); FederalOffice for Building and
DIN EN 13501-1 Fire classification of construction products and Regional Planning (BBSR), 2011: Nutzungsdauern von
building elements – Part 1: Classification using data from Bauteilen für Lebenszyklusanalysen nach Bewertungssystem
reaction to fire tests; German version EN 13501- Nachhaltiges Bauen (BNB) (Service lives of building elements
1:2007+A1:2009,2010-01 for Life Cycle Assessments conducted according to the BNB
Sustainable Building assessment system):
EN 15804
EN 15804:2012+A1:2013, Sustainability of construction works https://www.nachhaltigesbauen.de/fileadmin/pdf/baustoff_gebauededaten/BNB_Nutzungsdauern_von_Bauteilen_2017-
— Environmental Product Declarations — Core rules for the 2-24.pdf, dated: 24 February 2017
product category of construction products.
DepV and VVerDR
EN 15804 DepV (Landfill Ordinance) and VVerDR (Ordinance on
EN 15804:2012+A2:2019+AC:2021, Sustainability of Simplifying Landfill Law): 2009, German Federal Ministry of
construction works — Environmental Product Declarations — Justice and Consumer Protection, and Federal Office of Justice
Core rules for the product category of construction products. https://www.gesetze-im-internet.de/depv_2009/DepV.pdf, 27
April 2009
EN ISO 7783-2
EN ISO 7783-2:1999 Paints and varnishes– Coating materials ECOTOX Database
and coating systems for exterior masonry and concrete – Part ECOTOX Database https://cfpub.epa.gov/ecotox/, 2019-06
5 Environmental Product Declaration - Sto SE & Co. KGaA - StoVentec Carrier Board S
EWC LAGA EW 98 S
European Waste Catalogue (EWC); Regulation (EC) No. Bund/Länder-Arbeitsgemeinschaft Abfall (Federal/State
1272/2008 of the European Parliament and of the Council of 16 Working Group for Waste; LAGA) 33 https://www.umwelt-
December 2008 on classification, labelling and packaging of online.de/recht/abfall/laga/m33_ges.htm, September 2017
substances and mixtures, amending and repealing Directives
67/548/EEC and 1999/45/EC, and amending Regulation (EC) PCR Part A
No 1907/2006 PCR - Part A: Calculation Rules for the Life CycleAssessment
and Requirements on the Project Report,Berlin: Institut Bauen
GaBi ts documentation und Umwelt e.V., www.ibu-epd.com, Version 1.3, 2021
GaBi life cycle inventory data documentation
(https://www.gabisoftware.com/support/gabi/gabidatab PCR Part B
ase2020lcidocumentation/) PCR Part B: Product Category Rules for Building-Related
Products and Services. Part B: Requirements on the EPD for
GaBi ts software Lightweight boards made of lightweight fillers and reactive
Sphera Solutions GmbH GaBi Software System and Database resins, Version 3. Berlin: Institut Bauen und Umwelt e.V. (ed.),
for Life Cycle Engineering CUP Version: 2022.2 University of 2023.07.
Stuttgart Leinfelden Echterdingen
IBU 2021
Institut Bauen und Umwelt e.V.: General Programme
Instructions for the Preparation of EPDs at the Institut Bauen
und Umwelt e.V. Version 2.0, Berlin: Institut Bauen und Umwelt
e.V., 2021
6 Environmental Product Declaration - Sto SE & Co. KGaA - StoVentec Carrier Board S
Publisher
Institut Bauen und Umwelt e.V. +49 (0)30 3087748- 0
Hegelplatz 1 info@ibu-epd.com
10117 Berlin www.ibu-epd.com
Germany
Programme holder
Institut Bauen und Umwelt e.V. +49 (0)30 3087748- 0
Hegelplatz 1 info@ibu-epd.com
10117 Berlin www.ibu-epd.com
Germany
Author of the Life Cycle Assessment
Sphera Solutions GmbH +49 711 341817-0
Hauptstraße 111- 113 info@sphera.com
70771 Leinfelden-Echterdingen www.sphera.com
Germany
Owner of the Declaration
Sto SE & Co. KGaA +49 7744 57-1010
Ehrenbachstr. 1 infoservice@sto.com
79780 Stühlingen www.sto.com
Germany
7 Environmental Product Declaration - Sto SE & Co. KGaA - StoVentec Carrier Board S
