ENVIRONMENTAL PRODUCT DECLARATION
as per ISO 14025 and EN 15804+A2
Owner of the Declaration Hilti Aktiengesellschaft
Publisher Institut Bauen und Umwelt e.V. (IBU)
Programme holder Institut Bauen und Umwelt e.V. (IBU)
Declaration number EPD-HIL-20240046-CBA1-EN
Issue date 04.06.2024
Valid to 03.06.2029
HST4 Wedge anchor
HILTI AG
www.ibu-epd.com | https://epd-online.com
General Information
HILTI AG HST4 Wedge anchor
Programme holder Owner of the declaration
IBU – Institut Bauen und Umwelt e.V. Hilti Aktiengesellschaft
Hegelplatz 1 Feldkircher Strasse 100
10117 Berlin 9494 Schaan
Germany Liechtenstein
Declaration number Declared product / declared unit
EPD-HIL-20240046-CBA1-EN HST4 / 1kg
This declaration is based on the product category rules: Scope:
Screws, 01.06.2023 The document relates to the carbon steel HST4 portfolio as a leading Hilti
(PCR checked and approved by the SVR) wedge anchor product group. The HST4 wedge anchors portfolio consists
of a diameter range from M8 - M20 and a standard length portfolio of
50mm-260mm. The declared product for this specific EPD is the HST4
Issue date M10x90, which represents one of the most commonly used and produced
items in the carbon steel portfolio.
04.06.2024
The owner of the declaration shall be liable for the underlying information
and evidence; the IBU shall not be liable with respect to manufacturer
information, life cycle assessment data and evidences.
Valid to
03.06.2029 The EPD was created according to the specifications of EN 15804+A2. In
the following, the standard will be simplified as EN 15804.
Verification
The standard EN 15804 serves as the core PCR
Independent verification of the declaration and data according to ISO
14025:2011
internally X externally
Dipl.-Ing. Hans Peters
(Chairman of Institut Bauen und Umwelt e.V.)
Florian Pronold Matthias Klingler,
(Managing Director Institut Bauen und Umwelt e.V.) (Independent verifier)
1 Environmental Product Declaration - HILTI AG - HST4 Wedge anchor
Product
Product description/Product definition
HST4 is a performance concrete wedge expansion anchor Application
used to resist static and seismic structural loads in the The core use of the product is in various construction sites
construction industry (residential, industrial, infrastructure, etc.). including but not limited to commercial, residential, industrial
The HST4 carbon steel variant of the HST4 family is described and infrastructure. The main applications for the HST4 wedge
further in this report. anchor is in the structural connection of baseplates to concrete
For the placing of the product on the market in the European base materials, in instances like Structural Steel members,
Union European Free Trade Association EU/EFTA) (with the Handrails and Balustrades, Façade connections and
exception of Switzerland) Regulation (EU) No. 305/2011 (CPR) MEP/services connections.
applies. The product needs a declaration of performance taking
into consideration the following European Technical Approval Technical Data
ETA-21/0878 assessed based on EAD 330232-01-0601-v03 Performance data of the product in accordance with the
'Mechanical fasteners with variable embedment depth for use in declaration of performance with respect to its essential
concrete'. For the application and use the respective national characteristics according to ETA-21/0878 and the relevant
provisions apply product technical data sheets.
The Hilti HST4 anchor is a torque-controlled expansion anchor
made of carbon steel which is installed into a drilled hole and
Base materials/Ancillary materials
anchored by torque-controlled expansion
Reference service life
The lifetime of the HST4 mechanical fastener is defined by the
EAD 330232-01-0601-v03 and described in the ETA-21/0878
as referenced further.
The provisions made in this European technical assessment
are based on an assumed working life of the anchor of 50
years. The indications given on the working life cannot be
interpreted as a guarantee given by the producer but are to be
regarded only as a means for choosing the right products in
relation to the expected economically reasonable working life of
the works.
LCA: Calculation rules
Declared Unit
The declared product is the HST4 M10x90 5-40 from HILTI AG. Production stage (A1- A3):
The declared unit refers to 1 kg of bolt anchor. Packaging is - A1, raw material extraction,
also included in the calculation, as Hilti sells the product with - A2, transport to the manufacturer,
packaging. The declared unit is stated in [kg]. - A3, production.
Declared unit and mass reference
Name Value Unit
End of life (C1- C4):
Declared unit 1 kg
- C1, dismantling/demolition,
Gross density 7850 kg/m3 - C2, transport,
- C3, waste treatment ,
System boundary - C4, disposal.
Type of EPD: cradle to factory gate with options. The following
information modules are defined as system boundaries in this
study: Reuse, recovery and recycling potential (D)
2 Environmental Product Declaration - HILTI AG - HST4 Wedge anchor
In order to accurately record the indicators and environmental
impacts of the declared unit, a total of 8 information modules
are considered. The information modules A1 to A3 describe the Figure Information modules A 1 to A3 of the packaging
provision of materials, transport to the production site and the
production processes of the product itself. Information modules C1 to C4 record the dismantling or
demolition of the building, transport for waste disposal, waste
treatment and disposal of the product. Furthermore, reuse,
The primary products are sourced from the European Union. recovery and recycling potentials are shown in information
Transport is by lorry. The following flow charts illustrate the module D.
underlying production process.
Geographic Representativeness
Land or region, in which the declared product system is
manufactured, used or handled at the end of the product´s
lifespan: EU-27 Member States
Comparability
Basically, a comparison or an evaluation of EPD data is only
possible if all the data sets to be compared were created
according to EN 15804 and the building context, respectively
the product-specific characteristics of performance, are taken
Figure Information modules A 1 to A3 of the product
into account. The database referred to in this study is LCA for
Experts by Sphera.
LCA: Scenarios and additional technical information
The demolition of the bolt anchor from the building is calculated
Characteristic product properties of biogenic carbon in information module C1.The demolition is carried out using an
The declared product does not contain any biogenic electric chisel. The electrical energy consumption for the tool is
Carbon. assumed to be 0.5 MJ for the declared unit. The electricity
Information on describing the biogenic carbon content at consumption is calculated using a European electricity mix.
factory gate Name Value Unit
Name Value Unit Collected separately waste type waste type 1 kg
Biogenic carbon content in accompanying kg Recycling 0.85 kg
0.0028
packaging C Landfilling 0.15 kg
Note: 1 kg of biogenic carbon is equivalent to 44/12 kg of CO2
Reuse, recovery and/or recycling potentials (D), relevant
scenario information
In Module D, a recycling rate of 85% is assumed (world steel
association).
End of life (C1-C4)
Name Value Unit
Recycling 0,85 kg
3 Environmental Product Declaration - HILTI AG - HST4 Wedge anchor
LCA: Results
DESCRIPTION OF THE SYSTEM BOUNDARY (X = INCLUDED IN LCA; MND = MODULE OR INDICATOR NOT DECLARED; MNR
= MODULE NOT RELEVANT)
Benefits and
Construction loads beyond
Product stage Use stage End of life stage
process stage the system
boundaries
la ire ta m w a Ry lp p u s tro p s n a rT g n iru tc a fu n a M e h t m o rf tro p s n a rTe tis e h t o t e ta g y lb m e s s A e s U e c n a n e tn ia M ria p e R tn e m e c a lp e R tn e m h s ib ru fe R y g re n e la n o ita re p Oe s u re ta w la n o ita re p Oe s u n o itc u rts n o c -e Dn o itilo m e d tro p s n a rT g n is s e c o rp e ts a W la s o p s iD -e s u e R-y re v o c e R-g n ilc y c e Rla itn e to p
A1 A2 A3 A4 A5 B1 B2 B3 B4 B5 B6 B7 C1 C2 C3 C4 D
X X X MND MND MND MND MNR MNR MNR MND MND X X X X X
RESULTS OF THE LCA - ENVIRONMENTAL IMPACT according to EN 15804+A2: 1 kg
Parameter Unit A1-A3 C1 C2 C3 C4 D
Global Warming Potential total (GWP-total) kg CO 2 eq 2.77E+00 5.86E-02 3.73E-03 2.58E-03 2.2E-03 -1.7E+00
Global Warming Potential fossil fuels (GWP-fossil) kg CO 2 eq 2.77E+00 5.86E-02 3.7E-03 2.56E-03 2.19E-03 -1.7E+00
Global Warming Potential biogenic (GWP-biogenic) kg CO 2 eq 0 0 0 0 0 0
Global Warming Potential luluc (GWP-luluc) kg CO 2 eq 1.33E-03 5.36E-06 3.39E-05 1.92E-05 6.79E-06 -6.31E-04
Depletion potential of the stratospheric ozone layer (ODP) kg CFC11 eq 3.42E-12 5.76E-13 3.2E-16 4.28E-15 5.56E-15 -1.08E-12
Acidification potential of land and water (AP) mol H+ eq 5.63E-03 8.92E-05 4.03E-06 1.34E-05 1.55E-05 -3.9E-03
Eutrophication potential aquatic freshwater (EP-freshwater) kg P eq 1.99E-06 5.79E-08 1.33E-08 8.71E-09 4.4E-09 -1.28E-06
Eutrophication potential aquatic marine (EP-marine) kg N eq 1.45E-03 2.52E-05 1.36E-06 6.13E-06 4.01E-06 -9.58E-04
Eutrophication potential terrestrial (EP-terrestrial) mol N eq 1.58E-02 2.66E-04 1.61E-05 6.77E-05 4.41E-05 -1.03E-02
Formation potential of tropospheric ozone photochemical oxidants kg NMVOC
4.78E-03 6.95E-05 3.5E-06 1.66E-05 1.21E-05 -3.26E-03
(POCP) eq
Abiotic depletion potential for non fossil resources (ADPE) kg Sb eq 9.72E-08 2.84E-09 2.36E-10 2.74E-09 1.01E-10 -6.59E-08
Abiotic depletion potential for fossil resources (ADPF) MJ 2.93E+01 1.29E+00 4.97E-02 5.04E-02 2.91E-02 -1.43E+01
m3 world eq
Water use (WDP) 3.6E-02 4.92E-03 4.21E-05 4.98E-04 2.4E-04 -2.19E-02
deprived
RESULTS OF THE LCA - INDICATORS TO DESCRIBE RESOURCE USE according to EN 15804+A2: 1 kg
Parameter Unit A1-A3 C1 C2 C3 C4 D
Renewable primary energy as energy carrier (PERE) MJ 1.51E+00 1.76E-01 3.52E-03 4.68E-03 4.74E-03 -8.12E-01
Renewable primary energy resources as material utilization
MJ 2.9E-01 0 0 0 0 0
(PERM)
Total use of renewable primary energy resources (PERT) MJ 1.8E+00 1.76E-01 3.52E-03 4.68E-03 4.74E-03 -8.12E-01
Non renewable primary energy as energy carrier (PENRE) MJ 2.94E+01 1.29E+00 4.99E-02 5.05E-02 2.91E-02 -1.44E+01
Non renewable primary energy as material utilization (PENRM) MJ 0 0 0 0 0 0
Total use of non renewable primary energy resources (PENRT) MJ 2.94E+01 1.29E+00 4.99E-02 5.05E-02 2.91E-02 -1.44E+01
Use of secondary material (SM) kg 0 0 0 0 0 0
Use of renewable secondary fuels (RSF) MJ 0 0 0 0 0 0
Use of non renewable secondary fuels (NRSF) MJ 0 0 0 0 0 0
Use of net fresh water (FW) m3 4.62E-03 2.95E-04 3.88E-06 1.44E-05 7.35E-06 -1.96E-03
RESULTS OF THE LCA – WASTE CATEGORIES AND OUTPUT FLOWS according to EN 15804+A2:
1 kg
Parameter Unit A1-A3 C1 C2 C3 C4 D
Hazardous waste disposed (HWD) kg 9.8E-10 7.46E-11 1.84E-13 1.31E-13 6.34E-13 3.58E-10
Non hazardous waste disposed (NHWD) kg 2.91E-02 2.84E-04 7.18E-06 1.33E-05 1.46E-01 -2.12E-02
Radioactive waste disposed (RWD) kg 1.45E-03 2.01E-04 6.45E-08 6.77E-07 3.31E-07 -8.09E-05
Components for re-use (CRU) kg 0 0 0 0 0 0
Materials for recycling (MFR) kg 0 0 0 0 0 0
Materials for energy recovery (MER) kg 0 0 0 0 0 0
Exported electrical energy (EEE) MJ 0 0 0 0 0 0
Exported thermal energy (EET) MJ 0 0 0 0 0 0
RESULTS OF THE LCA – additional impact categories according to EN 15804+A2-optional:
1 kg
Parameter Unit A1-A3 C1 C2 C3 C4 D
Disease
Incidence of disease due to PM emissions (PM) ND ND ND ND ND ND
incidence
Human exposure efficiency relative to U235 (IR) kBq U235 eq ND ND ND ND ND ND
Comparative toxic unit for ecosystems (ETP-fw) CTUe ND ND ND ND ND ND
Comparative toxic unit for humans (carcinogenic) (HTP-c) CTUh ND ND ND ND ND ND
Comparative toxic unit for humans (noncarcinogenic) (HTP-nc) CTUh ND ND ND ND ND ND
4 Environmental Product Declaration - HILTI AG - HST4 Wedge anchor
Soil quality index (SQP) SQP ND ND ND ND ND ND
Disclaimer 1 – for the indicator “Potential Human exposure efficiency relative to U235”. This impact category deals mainly with the
eventual impact of low-dose ionizing radiation on human health of the nuclear fuel cycle. It does not consider effects due to possible
nuclear accidents, occupational exposure or radioactive waste disposal in underground facilities. Potential ionizing radiation from the
soil, radon and from some construction materials is also not measured by this indicator.
Disclaimer 2 – for the indicators “abiotic depletion potential for non-fossil resources”, “abiotic depletion potential for fossil resources”,
“water (user) deprivation potential, deprivation-weighted water consumption”, “potential comparative toxic unit for ecosystems”,
“potential comparative toxic unit for humans – cancerogenic”, “Potential comparative toxic unit for humans - not cancerogenic”,
“potential soil quality index”. The results of this environmental impact indicator shall be used with care as the uncertainties on these
results are high as there is limited experience with the indicator.
References
EN 15804
EN 15804:2012+A2:2019+AC:2021, Sustainability Produktkategorienregeln Teil B
ofconstruction works — Environmental Product Declarations — Screws, 01.06.2023
Core rules for the product category of construction products.
Sphera
ISO 14025 LCA for Experts: Ganzheitliche Bilanzierung Leinfelden-
EN ISO 14025:2011, Environmental labels and declarations — Echterdingen; Sphera Solution GmbH (Hrsg.)
Type III environmental declarations — Principles and www.gabi-software.com/deutsch/index/
procedures. (07.11.2023)
IBU 2021
General Instructions for the EPD programme of Institut Bauen EAD330232-01-0601-v03
und Umwelt e.V. Version 2.0, European Assessment Document - Mechanical fasteners for
Berlin: Institut Bauen und Umwelt e.V., 2021 use in concrete
www.ibu-epd.de
EN 10088-1:2014
Produktkategorienregeln Bauprodukte Teil A stainless steels - part 1: list of stainless steels
Produktkategorienregeln für Bauprodukte und
Dienstleistungen - Rechenregeln für die Ökobilanz und ETA-21/0878
Anforderungen an den Hintergrundbericht V1.3, Institut Bauen European Technical Assessment - Hilti HST4
und Umwelt e.V., 08.2022.
5 Environmental Product Declaration - HILTI AG - HST4 Wedge anchor
Publisher
Institut Bauen und Umwelt e.V. +49 (0)30 3087748- 0
Hegelplatz 1 info@ibu-epd.com
10117 Berlin www.ibu-epd.com
Germany
Programme holder
Institut Bauen und Umwelt e.V. +49 (0)30 3087748- 0
Hegelplatz 1 info@ibu-epd.com
10117 Berlin www.ibu-epd.com
Germany
Author of the Life Cycle Assessment
FIT-Umwelttechnik GmbH 05362 72 69 474
Westerstr. 13 bertram@fit-umwelttechnik.de
38442 Wolfsburg www.fit-umwelttechnik.com
Germany
Owner of the Declaration
Hilti Aktiengesellschaft +423 234 2111
Feldkircher Strasse 100 HAGHSE@hilti.com
9494 Schaan www.hilti.com
Liechtenstein
6 Environmental Product Declaration - HILTI AG - HST4 Wedge anchor
