ENVIRONMENTAL PRODUCT DECLARATION
as per ISO 14025 and EN 15804+A2
Owner of the Declaration dormakaba International Holding GmbH
Publisher Institut Bauen und Umwelt e.V. (IBU)
Programme holder Institut Bauen und Umwelt e.V. (IBU)
Declaration number EPD-DOR-20210209-CBA2-EN
Issue date 07.10.2021
Valid to 06.10.2026
Terminal 96 00
dormakaba
www.ibu-epd.com | https://epd-online.com
General Information
dormakaba Terminal 96 00
Programme holder Owner of the declaration
IBU – Institut Bauen und Umwelt e.V. dormakaba International Holding GmbH
Hegelplatz 1 DORMA Platz 1
10117 Berlin 58256 Ennepetal
Germany Germany
Declaration number Declared product / declared unit
EPD-DOR-20210209-CBA2-EN 1 piece of the product: Terminal 96 00
This declaration is based on the product category rules: Scope:
Electronic and physical Access Control Systems, 01.08.2021 This EPD refers to a specific product manufactured by dormakaba. The
(PCR checked and approved by the SVR) production site is located in Villingen-Schwenningen (Germany).
The data represents the year 2019.
Issue date The owner of the declaration shall be liable for the underlying information
and evidence; the IBU shall not be liable with respect to manufacturer
07.10.2021
information, life cycle assessment data and evidences.
The EPD was created according to the specifications of EN 15804+A2. In
Valid to
the following, the standard will be simplified as EN 15804.
06.10.2026
Verification
The standard EN 15804 serves as the core PCR
Independent verification of the declaration and data according to ISO
14025:2011
internally X externally
Dipl.-Ing. Hans Peters
(Chairman of Institut Bauen und Umwelt e.V.)
Florian Pronold Dr.-Ing. Wolfram Trinius,
(Managing Director Institut Bauen und Umwelt e.V.) (Independent verifier)
1 Environmental Product Declaration - dormakaba - Terminal 96 00
Product
- BLE (Android+iOS)
Product description/Product definition • CardLink to integrate offline door components
Secure and uncomplicated time recording with the terminal 96
00. A flexible, small all-rounder that you can expand later easily. Peripherals Interface
The user interface offers extensive configuration options to be • 4 digital inputs / 2 relay outputs via Add-On
adapted to your corporate identity featuring company-specific
content and applications. Its stable housing and robust glass Power supply
screen make the terminal durable and versatile in application. • PoE IEEE802.3at
The employee identification is done via integrated radio-
frequency identification (RFID) reader using an RFID medium Power class 0 (0.44–12.95 W)
or smartphone. For the placing on the market in the European
Union/European Free Trade Association (EU/EFTA, with the Installation
exception of Switzerland) the following legal provisions apply: • Wall mounting
• Radio Equipment Directive (RED) • Class of protection: IP20/IP65
• Restriction of Hazardous Substances (RoHS)
• EN 50581:2012 The product is not harmonised in accordance with the
The CE-marking takes into account the proof of conformity with Construction Product Regulations (CPR) but in accordance with
the respective harmonized standards based on the legal other provisions for harmonisation of the EU. Compliance with
provisions above. For the application and use the respective the European Union Directive and technical specifications:
national provisions apply. • EN 300330 V2.1.1
• EN 301489-1 V2.2.0
Application
• EN 301489-3 V2.1.1
• Attendance recording • EN 62311:2008
• Door Control • EN 62368-1:2014
• Staff Communication The product is subject to CE marking according to the relevant
harmonization legislation.
Technical Data In addition, the product also conforms to the following
The terminal 96 00 has the following technical properties: standards:
Name Value Unit • UL 62368-1:2014
Operating Temperature -25 - 55 °C • CAN/CSA-22.2 No. 62368-1:2014
Operating Humidity 5 - 85 % • FCC Part 15 Class C
Width Dimension 89 mm
Base materials/Ancillary materials
Height Dimension 177 mm
The major material compositions of the product are listed
Depth Dimension 32 mm below:
Weight (without packaging) 0,485 kg Name Value Unit
Weight (with packaging) 0,756 kg Paper 36 %
Power consumption "on mode" 12 W Aluminium 26 %
Power consumption "idle mode" 8 W Electronics 21 %
Power consumption "standby mode" 5 Plastics 15 %
Host Interface Glass 1 %
• Ethernet 10/100/1000BASE-T IEEE802.3 compatible Others 1 %
• Optional WLAN IEEE802.11 a/b/g/n (2,4/5 GHz)
The product includes partial articles which contain substances
listed in the Candidate List of REACH Regulation
User Interface
1907/2006/EC (date: 08.07.2021) exceeding 0.1 percentage by
• 4' illuminated touch screen display
mass: no
• Loudspeaker
• RFID reader
Reference service life
- MRD (LEGIC / MIFARE)
The reference service life of the dormakaba Terminal 96 00 is
- HID (iClass SE Prox)
estimated to be 10 years. This number is based on the support
• MAG stripe reader (optional)
and service life and is not an estimated lifetime.
• Booking via smartphone
- NFC (Android)
LCA: Calculation rules
Declared Unit System boundary
The declared unit is 1 piece of the product: Terminal 96 00. The type of EPD is: cradle to gate with options, modules C1–
C4, and module D (A1–A3 + C + D and additional modules: A4
Declared unit
+ A5 + B6)
Name Value Unit
Declared unit 1 pce. Production - Module A1-A3
Conversion factor to 1 kg (kg per declared unit) 1.32 - The product stage includes:
Product weight incuding packaging 0,756 kg — A1, raw material extraction, processing and mechanical
2 Environmental Product Declaration - dormakaba - Terminal 96 00
treatments, processing of secondary material input (e.g. — C3, waste processing for reuse, recovery and/or recycling;
recycling processes), — C4, disposal;
— A2, transport to the manufacturer, including provision and all transport, provision of all materials,
— A3, manufacturing and assembly products and related energy and water use.
including provision of all materials, products and energy, as well
as waste processing up to the end-of waste state. Module D (Benefits and loads beyond the system boundary)
includes:
Construction stage - Modules A4-A5 — D, recycling potentials, expressed as net impacts and
The construction process stage includes: benefits.
— A4, transport to the building site;
— A5, installation into the building; Geographic Representativeness
including provision of all materials, products and energy, as well Land or region, in which the declared product system is
as waste processing up to the end-of-waste state or disposal of manufactured, used or handled at the end of the product´s
final residues during the construction process stage. lifespan: Germany
Use stage - Module B6
Comparability
The use stage related to the operation of the building includes:
Basically, a comparison or an evaluation of EPD data is only
— B6, operational energy use
possible if all the data sets to be compared were created
according to EN 15804 and the building context, respectively
End-of-life stage– Modules C1-C4 and D
the product-specific characteristics of performance, are taken
The end-of-life stage includes:
into account. Background database: GaBi, SP40.
— C1, de-construction, demolition:
— C2, transport to waste processing;
LCA: Scenarios and additional technical information
Operational energy use (B6) and Operational water use
Characteristic product properties of biogenic carbon
(B7)
Information on describing the biogenic Carbon Content at The use stage is declared for 15 years.
factory gate
Name Value Unit
Name ValueUnit
Energy consumption for 1 year 48.9 kWh
Biogenic carbon content in accompanying kg
0.1 on mode per day 1 h
packaging C
idle mode 3 h
Note: 1 kg of biogenic carbon is equivalent to 44/12 kg of CO .
2 on mode power 12 W
idle mode 8 W
Days per year in use 365 days
The following technical scenario information is required for the
declared modules.
End of life (C1-C4)
Transport to the building site (A4) C1: The product dismantling from the building is done manually
Name Value Unit without environmental burden.
Litres of fuel per 1 kg (truck) 0.00276 l/100km Name Value Unit
Transport distance (truck) 1200 km Collected separately waste type 0.485 kg
Transport distance (ship) 20500 km Recycling 0.349 kg
Capacity utilisation (including empty runs) 55 % Energy recovery 0.111 kg
Final deposition 0,0253 kg
Installation into the building (A5)
Transportation to Waste Processing Site 50 km
Name Value Unit
Region for end of life: Global
Waste Packaging (paper) 0,2705 kg
Reference service life Reuse, recovery and/or recycling potentials (D), relevant
scenario information
Name Value Unit
Collection rate is 100%.
Life Span according to the manufacturer 10 a
3 Environmental Product Declaration - dormakaba - Terminal 96 00
LCA: Results
DESCRIPTION OF THE SYSTEM BOUNDARY (X = INCLUDED IN LCA; MND = MODULE OR INDICATOR NOT DECLARED; MNR
= MODULE NOT RELEVANT)
Benefits and
Construction loads beyond
Product stage Use stage End of life stage
process stage the system
boundaries
la ire ta m w a Ry lp p u s tro p s n a rT g n iru tc a fu n a M e h t m o rf tro p s n a rTe tis e h t o t e ta g y lb m e s s A e s U e c n a n e tn ia M ria p e R tn e m e c a lp e R tn e m h s ib ru fe R y g re n e la n o ita re p Oe s u re ta w la n o ita re p Oe s u n o itc u rts n o c -e Dn o itilo m e d tro p s n a rT g n is s e c o rp e ts a W la s o p s iD -e s u e R-y re v o c e R-g n ilc y c e Rla itn e to p
A1 A2 A3 A4 A5 B1 B2 B3 B4 B5 B6 B7 C1 C2 C3 C4 D
X X X X X MND MND MNR MNR MNR X MND X X X X X
RESULTS OF THE LCA - ENVIRONMENTAL IMPACT according to EN 15804+A2: 1 piece Terminal 96 00
Parameter Unit A1-A3 A4 A5 B6 C1 C2 C3 C4 D
GWP-total kg CO 2 eq 4.76E+01 1.02E-01 3.17E+00 3.28E+02 0 3.83E-02 1.44E-01 2.8E-02 -2.31E+00
GWP-fossil kg CO 2 eq 5.02E+01 9.76E-02 1.29E-01 3.26E+02 0 3.66E-02 1.44E-01 2.79E-02 -2.31E+00
GWP-biogenic kg CO 2 eq -2.72E+00 4.51E-03 3.04E+00 1.09E+00 0 1.69E-03 3.35E-06 9.52E-05 1.26E-03
GWP-luluc kg CO 2 eq 7E-02 2.32E-06 5.42E-05 4.73E-01 0 8.72E-07 8.13E-06 8.02E-05 -3.17E-03
ODP kg CFC11 eq 3.49E-09 1.03E-17 5.88E-16 7.18E-12 0 3.87E-18 7.26E-17 1.03E-16 -1.71E-14
AP mol H+ eq 3E-01 9.77E-05 8.83E-04 7.2E-01 0 3.67E-05 2.56E-05 2E-04 -2.54E-02
EP-freshwater kg P eq 3.38E-04 2.09E-08 1.14E-07 8.71E-04 0 7.84E-09 1.16E-08 4.78E-08 -2.34E-06
EP-marine kg N eq 4.55E-02 3.11E-05 3.17E-04 1.6E-01 0 1.17E-05 5.78E-06 5.14E-05 -2.06E-03
EP-terrestrial mol N eq 4.82E-01 3.46E-04 3.97E-03 1.68E+00 0 1.3E-04 1.17E-04 5.65E-04 -2.22E-02
kg NMVOC
POCP 1.37E-01 8.79E-05 8.42E-04 4.38E-01 0 3.3E-05 1.6E-05 1.56E-04 -6.72E-03
eq
ADPE kg Sb eq 1.06E-02 2.93E-09 9.23E-09 9.44E-05 0 1.1E-09 9.95E-10 2.5E-09 -1.13E-03
ADPF MJ 6.11E+02 1.38E+00 1.01E+00 5.73E+03 0 5.2E-01 6.67E-02 3.66E-01 -3.37E+01
m3 world eq
WDP 1.35E+01 1.91E-04 3.92E-01 7.11E+01 0 7.18E-05 1.47E-02 2.92E-03 -7.74E-01
deprived
GWP = Global warming potential; ODP = Depletion potential of the stratospheric ozone layer; AP = Acidification potential of land and water; EP =
Eutrophication potential; POCP = Formation potential of tropospheric ozone photochemical oxidants; ADPE = Abiotic depletion potential for non-fossil
resources; ADPF = Abiotic depletion potential for fossil resources; WDP = Water (user) deprivation potential)
RESULTS OF THE LCA - INDICATORS TO DESCRIBE RESOURCE USE according to EN 15804+A2: 1 piece Terminal 96 00
Parameter Unit A1-A3 A4 A5 B6 C1 C2 C3 C4 D
PERE MJ 1.56E+02 4.36E-03 2.66E+01 2.54E+03 0 1.64E-03 3.16E-02 4.79E-02 -6.31E+00
PERM MJ 2.64E+01 0 -2.64E+01 0 0 0 -1.43E-02 0 0
PERT MJ 1.83E+02 4.36E-03 1.85E-01 2.54E+03 0 1.64E-03 1.73E-02 4.79E-02 -6.31E+00
PENRE MJ 6.04E+02 1.39E+00 1.87E+00 5.74E+03 0 5.2E-01 6.45E+00 3.66E-01 -3.37E+01
PENRM MJ 7.24E+00 0 -8.6E-01 0 0 0 -6.38E+00 0 0
PENRT MJ 6.12E+02 1.39E+00 1.01E+00 5.74E+03 0 5.2E-01 6.67E-02 3.66E-01 -3.37E+01
SM kg 7.49E+00 0 0 0 0 0 0 0 0
RSF MJ 0 0 0 0 0 0 0 0 0
NRSF MJ 0 0 0 0 0 0 0 0 0
FW m3 3.29E-01 7.83E-06 9.23E-03 2.94E+00 0 2.94E-06 3.52E-04 9.22E-05 -1.65E-02
PERE = Use of renewable primary energy excluding renewable primary energy resources used as raw materials; PERM = Use of renewable primary
energy resources used as raw materials; PERT = Total use of renewable primary energy resources; PENRE = Use of non-renewable primary energy
excluding non-renewable primary energy resources used as raw materials; PENRM = Use of non-renewable primary energy resources used as raw
materials; PENRT = Total use of non-renewable primary energy resources; SM = Use of secondary material; RSF = Use of renewable secondary fuels;
NRSF = Use of non-renewable secondary fuels; FW = Use of net fresh water
RESULTS OF THE LCA – WASTE CATEGORIES AND OUTPUT FLOWS according to EN 15804+A2:
1 piece Terminal 96 00
Parameter Unit A1-A3 A4 A5 B6 C1 C2 C3 C4 D
HWD kg 2.87E-05 1.34E-10 1.54E-09 2.37E-06 0 5.04E-11 2.54E-10 5.57E-09 1.06E-07
NHWD kg 3.11E+00 1.42E-04 1.03E-01 4.07E+00 0 5.32E-05 1.49E-02 1.84E+00 -3.36E-01
RWD kg 1.71E-02 1.49E-06 5.26E-05 8.7E-01 0 5.58E-07 2.48E-06 4.16E-06 -1.51E-03
CRU kg 0 0 0 0 0 0 0 0 0
MFR kg 0 0 0 0 0 0 7.38E+00 0 0
MER kg 0 0 0 0 0 0 0 0 0
EEE MJ 8.58E-01 0 4.81E+00 0 0 0 0 0 0
EET MJ 1.56E+00 0 8.77E+00 0 0 0 0 0 0
HWD = Hazardous waste disposed; NHWD = Non-hazardous waste disposed; RWD = Radioactive waste disposed; CRU = Components for re-use;
MFR = Materials for recycling; MER = Materials for energy recovery; EEE = Exported electrical energy; EET = Exported thermal energy
4 Environmental Product Declaration - dormakaba - Terminal 96 00
RESULTS OF THE LCA – additional impact categories according to EN 15804+A2-optional:
1 piece Terminal 96 00
Parameter Unit A1-A3 A4 A5 B6 C1 C2 C3 C4 D
Disease
PM 3.07E-06 5.14E-10 4.95E-09 6.04E-06 0 1.93E-10 3.27E-10 2.47E-09 -2.05E-07
incidence
IR kBq U235 eq 1.69E+00 2.13E-04 8.09E-03 1.43E+02 0 7.98E-05 2.23E-04 4.28E-04 -2.44E-01
ETP-fw CTUe 2.96E+02 9.81E-01 4.76E-01 2.45E+03 0 3.68E-01 2.5E-02 2.09E-01 -1.49E+01
HTP-c CTUh 4.17E-08 1.85E-11 2.55E-11 6.78E-08 0 6.93E-12 2.17E-12 3.09E-11 -1.07E-09
HTP-nc CTUh 1.08E-06 7.89E-10 1.15E-09 2.5E-06 0 2.96E-10 2.19E-10 3.41E-09 -7.13E-08
SQP SQP 5.44E+02 3.56E-03 2.68E-01 1.83E+03 0 1.34E-03 2E-02 7.62E-02 -1.34E+01
PM = Potential incidence of disease due to PM emissions; IR = Potential Human exposure efficiency relative to U235; ETP-fw = Potential comparative
Toxic Unit for ecosystems; HTP-c = Potential comparative Toxic Unit for humans (cancerogenic); HTP-nc = Potential comparative Toxic Unit for humans
(not cancerogenic); SQP = Potential soil quality index
Disclaimer 1 – for the indicator IRP
This impact category deals mainly with the eventual impact of low dose ionizing radiation on human health of the nuclear fuel cycle. It
does not consider effects due to possible nuclear accidents, occupational exposure nor due to radioactive waste disposal in
underground facilities. Potential ionizing radiation from the soil, from radon and from some construction materials is also not measured
by this indicator.
Disclaimer 2 – for the indicators ADPE, ADPF, WDP, ETP-fw, HTP-c, HTP-nc, SQP
The results of this environmental impact indicator shall be used with care as the uncertainties on these results are high or as there is
limited experience with the indicator.
References
Standards
EN 62368-1
CAN/CSA-22.2 No. 62368-1 EN 62368-1:2014, Audio/video, information and communication
CAN/CSA-22.2 No. 62368-1:2014, Audio/video, information and technology equipment - Part 1: Safety requirements.
communication technologyequipment — Part 1: Safety
requirements. FCC Part 15 Class C
RADIO FREQUENCY DEVICES.
EN 15804+A2
EN 15804:2019+A2 (in press), Sustainability of construction ISO 14025
works — Environmental Product Declarations — Core rules for DIN EN ISO 14025:2011-10, Environmental labels and
the product category of construction products. declarations — Type III environmental declarations —
Principles and procedures.
EN 300330
EN 300330:2017, Short Range Devices (SRD) - Radio Radio Equipment Directive (RED)
equipment in the frequency range 9 kHz to 25 MHz and Directive 2014/53/EU of the European Parliament and of the
inductive loop systems in the frequency range 9 kHz to 30 Council of 16 April 2014 on the harmonisation of the laws of the
MHz - Harmonised Standard covering the essential Member States relating to the making available on the market
requirements of article 3.2 of the Directive 2014/53/EU. of radio equipment and repealing Directive 1999/5/EC.
EN 301489-1 Registration, Evaluation, Authorisation and Restriction of
EN 301489-1:2017, ElectroMagnetic Compatibility (EMC) Chemicals (REACH)
standard for radio equipment and services - Part 1: Common Regulation (EC) No 1907/2006 of the European Parliament and
technical requirements - Harmonised Standard covering the of the Council on the Registration, Evaluation, Authorisation
essential requirements of article 3.1(b) of Directive 2014/53/EU and Restriction of Chemicals (REACH).
and the essential requirements of article 6 of Directive
2014/30/EU. Restriction of Hazardous Substances (RoHS)
Directive on the restriction of the use of certain
EN 301489-3 hazardous substances in electrical and electronic
EN 301489-3:2017, ElectroMagnetic Compatibility (EMC) equipment (RoHS), Directive (EU) No 2011/65.
standard for radio equipment and services; Part 3: Specific
conditions for Short-Range Devices (SRD) operating on UL 62368-1
frequencies between 9 kHz and 246 GHz; Harmonised UL 62368-1:2014, Standard for Audio/video, information and
Standard covering the essential requirements of article 3.1(b) of communication technology equipment - Part 1: Safety
Directive 2014/53/EU. requirements.
EN 50581 Further References
EN 50581:2012, Technical documentation for the assessment
of electrical and electronic products with respect to the IBU 2016
restriction of hazardous substances. Institut Bauen und Umwelt e.V.: General Instructions for the
EPD programme of Institut Bauen und Umwelt e.V. Version 2.0,
EN 62311 Berlin: Institut Bauen und Umwelt e.V., 2021.
EN 62311:2008, Assessment of electronic and electrical
equipment related to human exposure restrictions for GaBi ts software
electromagnetic fields. Sphera Solutions GmbH
5 Environmental Product Declaration - dormakaba - Terminal 96 00
Gabi Software System and Database for Life Cycle Engineering
1992-2020 Version 10.0.0.71 University of Stuttgart Leinfelden- PCR Part A
Echterdingen PCR – Part A:
Calculation Rules for the Life Cycle As-sessment and
GaBi ts documentation Requirements on the Project Re-port according to EN
GaBi life cycle inventory data documentation (https://www.gabi- 15804+A2:2019, Version 1.0, Institut Bauen und Umwelt e.V.,
software.com/support/gabi/gabi-database-2020-lci- www.ibu-epd.com.
documentation/).
PCR Part B
LCA-tool dormakaba PCR – Part B: Requirements on the EPD for Building Hardware
LCA tool, version 1.0. product, version 1.3, Institut Bauen und Umwelt e.V., www.ibu-
Developed by Sphera Solutions GmbH. epd.com, 2019.
6 Environmental Product Declaration - dormakaba - Terminal 96 00
Publisher
Institut Bauen und Umwelt e.V. +49 (0)30 3087748- 0
Hegelplatz 1 info@ibu-epd.com
10117 Berlin www.ibu-epd.com
Germany
Programme holder
Institut Bauen und Umwelt e.V. +49 (0)30 3087748- 0
Hegelplatz 1 info@ibu-epd.com
10117 Berlin www.ibu-epd.com
Germany
Author of the Life Cycle Assessment
Sphera Solutions GmbH +49 711 341817-0
Hauptstraße 111- 113 info@sphera.com
70771 Leinfelden-Echterdingen www.sphera.com
Germany
Owner of the Declaration
dormakaba International Holding GmbH +49 2333 793-0
DORMA Platz 1 info.de@dormakaba.com
58256 Ennepetal www.dormakaba.com
Germany
7 Environmental Product Declaration - dormakaba - Terminal 96 00
