ENVIRONMENTAL PRODUCT DECLARATION
as per ISO 14025 and EN 15804+A2
Owner of the Declaration Knauf Ceiling Solutions GmbH & Co. KG
Publisher Institut Bauen und Umwelt e.V. (IBU)
Programme holder Institut Bauen und Umwelt e.V. (IBU)
Declaration number EPD-KNA-20240024-IBI1-EN
Issue date 12.03.2024
Valid to 11.03.2029
Classic Lite
Knauf Ceiling Solutions GmbH & Co. KG
www.ibu-epd.com | https://epd-online.com
1. General Information
Knauf Ceiling Solutions GmbH & Co. KG Classic Lite
Programme holder Owner of the declaration
IBU – Institut Bauen und Umwelt e.V. Knauf Ceiling Solutions GmbH & Co. KG
Hegelplatz 1 Elsenthal 15
10117 Berlin 94481 Grafenau
Germany Germany
Declaration number Declared product / declared unit
EPD-KNA-20240024-IBI1-EN 1 m² Classic Lite mineral ceiling tiles with a surface weight of 3.52 kg/m²,
equal to 1 m² of Fine Fissured mineral ceiling tiles with a surface weight of
3.52 kg/m², representative for 1 m² of Dune mineral ceiling tiles with a
surface weight of 3.36 kg/m²
This declaration is based on the product category rules: Scope:
Mineral panels, 01.08.2021 This document refers to 1 m² Classic Lite mineral ceiling tiles with a
(PCR checked and approved by the SVR) surface weight of 3.52 kg/m², manufactured at the production facility in
Wujiang, China.
Results for Classic Lite are also representative for 1 m² of Fine Fissured
Issue date mineral ceiling tiles with a surface weight of 3.52 kg/m² and for 1 m² of
Dune mineral ceiling tiles with a surface weight of 3.36 kg/m²
12.03.2024
(overestimation of environmental impacts of about 3 %), both
manufactured at the production facility in Wujiang, China.
Valid to
The owner of the declaration shall be liable for the underlying information
11.03.2029 and evidence; the IBU shall not be liable with respect to manufacturer
information, life cycle assessment data and evidences.
The EPD was created according to the specifications of EN 15804+A2. In
the following, the standard will be simplified as EN 15804.
Verification
The standard EN 15804 serves as the core PCR
Independent verification of the declaration and data according to ISO
14025:2011
internally X externally
Dipl.-Ing. Hans Peters
(Chairman of Institut Bauen und Umwelt e.V.)
Florian Pronold Vito D'Incognito,
(Managing Director Institut Bauen und Umwelt e.V.) (Independent verifier)
1 Environmental Product Declaration - Knauf Ceiling Solutions GmbH & Co. KG - Classic Lite
2. Product
exceeding 0.1 percentage by mass: No.
2.1 Product description/Product definition
The ceiling tiles are manufactured using a wet-felt process and This product/article/at least one partial article contains other
consist of biosoluble mineral wool, perlite, clay and starch. In carcinogenic, mutagenic, reprotoxic (CMR) substances in
addition, the visible side of the mineral tile is painted with categories 1A or 1B which are not on the candidate list,
dispersion paint. The back side is primed with dispersion paint. exceeding 0.1 percentage by mass: No.
The mineral tiles are available in different formats and edge Biocide products were added to this construction product or it
finishes. has been treated with biocide products (this then concerns a
treated product as defined by the (EU) Ordinance on Biocide
This EPD applies to the following products: Products No. 528/2012): No.
Classic Lite
Dune In-can preservatives are used in the production process;
Fine Fissured however, they are not part of the products and are therefore not
within the scope of the Ordinance on Biocide Products.
For the use and application of the product, the respective
national provisions at the place of use apply, in Germany for 2.6 Manufacture
example the building codes of the federal states and the The mineral tiles are produced in the traditional wet process
corresponding national specifications. (wet-felt). The raw materials are mixed with water to form a
homogeneous suspension, which is pumped onto a belt
2.2 Application conveyor (Fourdrinier). The water is removed mechanically
Mineral tiles (wet-felt) are typically used as lay-in for suspended (gravity and vacuum) and by evaporation in the drying oven. As
ceiling constructions. They are primarily used as optical far as possible, the process water is reused. It is treated
cladding, but also for sound absorption and sound insulation, accordingly and fed back into the process water circuit.
for fire resistance and against fire spreading, for cleanrooms Production waste and dust are reused in the process in the
and high hygiene requirements. sense of an internal cycle. The manufacturing plant is certified
according to ISO 9001, ISO 14001 and ISO 45001.
2.3 Technical Data
2.7 Environment and health during manufacturing
Construction data • The manufacturing plant is certified according to ISO
Name Value Unit 9001, ISO 14001 and ISO 45001.
• The production has a closed water cycle.
Noise reduction coefficient acc. ISO 354 and
0.55 • Production generates almost no waste, resulting blanks,
ASTM C 423-01
dust and rejects are reused.
Airborne Sound Attenuation acc. ISO 10848 and
33 dB • Not subject to declaration according to REACH.
ASTM E1414-11a
Formaldehyde emissions acc. ASTM D5116-17 0.0919mg/m3 2.8 Product processing/Installation
TVOC acc.ASTM D5116-17 <0.02 mg/m3 There are no recognised systemic hazards associated with the
installation of ceiling tiles. It is recommended that materials are
handled in a manner that minimises dust generation. Workers
Performance data of the product with respect to its
should wear appropriate personal protective equipment.
characteristics in accordance with the relevant technical
Equipment such as gloves, goggles and dust masks are
provision (no CE-marking).
recommended to minimise exposure to dust and prevent skin
irritation.
2.4 Delivery status
The EPD refers to panels with a thickness of 16mm which can 2.9 Packaging
have variable length and width dimensions.
The panels are packaged in cardboard boxes and sealed with
transparent polyethylene film. These packages lie on
2.5 Base materials/Ancillary materials
chemically untreated wooden pallets. The pallets are wrapped
Mineral tile composition: with polyethylene stretch film. Foil, paper and wood can be
Name Value Unit recycled in the usual ways.
Mineral wool 22 %
2.10 Condition of use
Perlite 29 %
When handled properly, the mechanical and structural-physical
Clay 13 % properties of the mineral tile remain intact throughout its entire
Paper 6 % service life. Direct contact with water should be avoided due to
Starch 4 % the water-soluble binding agent starch.
Brokes/dust (internally looped production waste) 26 % 2.11 Environment and health during use
When properly installed, no dust/particles are released during
In addition, the visible side of the mineral tile is painted with the use phase. For the substance groups formaldehyde, volatile
dispersion paint. The back side is primed with a dispersion organic compounds (VOCs) and total volatile organic
paint. compounds (TVOCs), the limits according to ASTM D5116-17
The recycled content is not less than 28 %. are complied with.
This product/article/at least one partial article contains
substances listed in the ECHA-candidate list (date: 25.06.2020)
2 Environmental Product Declaration - Knauf Ceiling Solutions GmbH & Co. KG - Classic Lite
demand (COD) and biological oxygen demand (BOD).
2.12 Reference service life
The service life of the mineral tiles (wet-felted) is up to Mechanical destruction
50 years, depending on the area of use, exposure and state of The mineral slabs (wet-felt) can be broken by hand and also
maintenance. Within the framework of the conditions of use, no damaged superficially, which can result in minor dust formation.
ageing effects are to be expected apart from visual
discolouration caused by air circulation. 2.14 Re-use phase
If the panels are removed properly, they can be reinstalled. In
2.13 Extraordinary effects case of minor damage, the slabs can be reused as cut-to-size
Fire tiles. Mineral tiles can be returned to the manufacturing process
The specified product has been tested to comply with both if they are of the correct type and have sufficient material
British and American standards, meeting class 0 (BS 476) and quality; they can be recycled up to 100 %.
class 1 (ASTM E 84) requirements.
Name Value 2.15 Disposal
The waste code number of production residues for mineral tiles
Building material class ASTM E84 Class A
according to the AVV, German List of Wastes Ordinance is 10
Building material class BS 476 Class 0
11 03, the waste code number for construction site waste
(offcuts) is 17 06 04. If the tiles are not recycled as described in
Water 2.14., they are disposed of in a landfill.
In the case of prolonged contact with water, the starch binder
dissolves, which can lead to a loss of structure, and if the 2.16 Further information
soluble components are discharged into the sewage treatment Further information at www.knaufceilingsolutions.com
plant, they are biodegradable, increasing the chemical oxygen
3. LCA: Calculation rules
declaring a 50 km radius to the landfill. In reality, this scenario
3.1 Declared Unit may vary depending on the actual location of deconstruction
This EPD refers to a declared unit of 1 m² Classic Lite mineral and referring waste treatment.
ceiling tiles with a surface weight of 3.52 kg/m².
Declared Unit Module C3 | Waste processing
The declared scenario assumes landfilling of the product.
Name Value Unit
Referring environmental impacts are accounted for in module
Declared unit 1 m2 C4.
Grammage (with coating) 3.52 kg/m2
Layer thickness 0.016 m Module C4 | Disposal
Module C4 refers to the emissions from the disposal of the
Boardmill density (raw board, without coating) 215 kg/m³
acoustic board mineral ceiling tiles. The chosen scenario,
therefore, includes the environmental burdens of landfilling the
The ceiling tiles are produced at the Knauf Ceiling Solutions product.
production site in Wujiang, China.
Various types of mineral ceiling tiles are produced at the site. Module D | Benefits and loads beyond the system
Product-specific results are also representative for 1 m² of Fine boundary
Fissured mineral ceiling tiles with a surface weight of 3.52 The declared scenario assumes landfilling of the product.
kg/m². For 1 m² of Dune mineral ceiling tiles with a surface Referring environmental impacts are accounted for in module
weight of 3.36 kg/m² the results based on Classic Lite show an C4.
overestimation of environmental impacts of about 3 %.
3.3 Estimates and assumptions
3.2 System boundary Assumptions and approximations are applied in case of a lack
The life cycle assessment of Classic Lite mineral ceiling tiles of representative data. All assumptions and approximations are
includes a cradle-to-gate analysis of the products' documented precisely and represent a best-guess
environmental impacts with modules (A1–A3, C, D). representation of reality. In case of uncertainty, a conservative
Subsequent life cycle phases are part of the analysis: approach is chosen.
Module A1–A3 | Production stage This study builds on Chinese background data as far as
The production stage includes the upstream burdens of raw supported by the available databases. Nevertheless, some
material supply, their transports and the manufacturing plant of upstream supply chains of used raw materials were
Knauf Ceiling Solutions located in Wujiang (China). Mineral approximated via European data, due to a lack of
ceiling tiles are produced in the wet-felt process. Main raw geographically adapted datasets.
material inputs, therefore, refer to mineral wool, perlite, clay and
starch. The production site is supplied with electricity from the 3.4 Cut-off criteria
Chinese power grid and thermal energy from natural gas. The LCA model covers all available input and output flows,
which can be represented based on robust data. Data gaps are
Module C1 | Deconstruction and demolition filled with conservative assumptions from average data (when
Disassembly of the product is done either manually or using available) or with generic data and are documented
smaller tools. Referring energy demand is considered to be accordingly. Only data with a contribution lower than 1 % were
negligible. cut off. Thus, no data were neglected, of which a substantial
impact is to be expected. All relevant data were collected
Modul C2 | Transport to disposal comprehensively. Cut-off material and energy flows were
The transport to the disposal of the material is estimated chosen carefully based on their expected quantitative
3 Environmental Product Declaration - Knauf Ceiling Solutions GmbH & Co. KG - Classic Lite
contribution as well as potential environmental impacts. Thus, it basis.
can be assumed that the sum of all neglected input flows does
not account for more than 5 % of the total material, water and 3.8 Geographic Representativeness
energy flows. Land or region, in which the declared product system is
manufactured, used or handled at the end of the product´s
3.5 Background data lifespan: China
This study uses generic background data for the evaluation of
upstream environmental impacts from GaBi databases (GaBi
3.9 Allocation
10; 2022.2).
All information for the allocation of given material and energy
3.6 Data quality flows is based on site-related evaluations. The calculation of
Data collection is based on product-specific questionnaires. It specific input quantities for the raw board production is based
follows an iterative process of clarifying questions via e-mail, on the respective recipe. In addition, product-specific
telephone calls or in personal/web meetings. Intensive application rates (e.g. backcoat, primer, etc.) were available.
discussions between Knauf Ceiling Solutions and Daxner & Total annual energy consumption and waste flows are allocated
Merl result in an accurate mapping of product-related material based on the production share of the product.
and energy flows. This leads to a high quality of foreground
data collected. Data collection relies on a consistent process For in the production used waste paper, the system boundary is
according to ISO 14044. set after sorting. It is assumed that the end-of-waste status has
been reached. The system boundary for secondary raw
The technological, geographical and time-related materials defined in EN 15804 applies.
representativeness of the database was kept in mind when
3.10 Comparability
selecting background data. Whenever specific data were
missing, either generic datasets or representative average data Basically, a comparison or an evaluation of EPD data is only
were used instead. The implemented GaBi background possible if all the data sets to be compared were created
datasets refer to the latest versions available (not more than according to EN 15804 and the building context, respectively
ten years old) and are carefully chosen. the product-specific characteristics of performance, are taken
into account.
3.7 Period under review
Foreground data were collected in the 2021 production year, The GaBi background database was used to calculate the LCA
and the data are based on the volumes produced on an annual (GaBi 10; 2022.2).
4. LCA: Scenarios and additional technical information
Characteristic product properties of biogenic carbon
The biogenic carbon content quantifies the amount of biogenic
carbon in the declared product.
Installation in building (A5)
Information on the description of the biogenic carbon The End-of-Life of the product packaging materials is not
content at the factory gate declared in module A5.
Name ValueUnit
kg Name Value Unit
Biogenic carbon content in product 0.19
C Packaging (cardboard) 0.009 kg/m²
Biogenic carbon content in accompanying 0.015 kg Packaging (PE-film) 0.035 kg/m²
packaging C
End-of-Life (C1–C4)
The carbon stored in the packaging was taken into account as
"CO -neutral". Thus the storage effect of the carbon bound in Name Value Unit
2
the packaging is not included in the calculation but is Collected separately 3.52 kg
considered as emitted immediately. Landfilling 3.52 kg
4 Environmental Product Declaration - Knauf Ceiling Solutions GmbH & Co. KG - Classic Lite
5. LCA: Results
The following table contains the LCA results for a declared unit of 1 m² Classic Lite mineral ceiling tiles with a surface weight of
3.52 kg/m².
DESCRIPTION OF THE SYSTEM BOUNDARY (X = INCLUDED IN LCA; MND = MODULE OR INDICATOR NOT DECLARED; MNR
= MODULE NOT RELEVANT)
Benefits and
Construction loads beyond
Product stage Use stage End of life stage
process stage the system
boundaries
la ire ta m w a Ry lp p u s tro p s n a rT g n iru tc a fu n a M e h t m o rf tro p s n a rTe tis e h t o t e ta g y lb m e s s A e s U e c n a n e tn ia M ria p e R tn e m e c a lp e R tn e m h s ib ru fe R y g re n e la n o ita re p Oe s u re ta w la n o ita re p Oe s u n o itc u rts n o c -e Dn o itilo m e d tro p s n a rT g n is s e c o rp e ts a W la s o p s iD -e s u e R-y re v o c e R-g n ilc y c e Rla itn e to p
A1 A2 A3 A4 A5 B1 B2 B3 B4 B5 B6 B7 C1 C2 C3 C4 D
X X X MND MND MND MND MNR MNR MNR MND MND X X X X X
RESULTS OF THE LCA - ENVIRONMENTAL IMPACT according to EN 15804+A2: 1 m² Classic Lite ceiling tiles (3.52 kg/m²)
Parameter Unit A1-A3 C1 C2 C3 C4 D
Global Warming Potential total (GWP-total) kg CO 2 eq 1.74E+01 0 1.1E-02 0 7.45E-01 0
Global Warming Potential fossil fuels (GWP-fossil) kg CO 2 eq 1.81E+01 0 1.06E-02 0 5.25E-02 0
Global Warming Potential biogenic (GWP-biogenic) kg CO 2 eq -6.79E-01 0 4.68E-04 0 6.92E-01 0
Global Warming Potential luluc (GWP-luluc) kg CO 2 eq 1.26E-02 0 2.75E-07 0 9.7E-05 0
Depletion potential of the stratospheric ozone layer (ODP) kg CFC11 eq 1.66E-10 0 1.04E-15 0 1.23E-13 0
Acidification potential of land and water (AP) mol H+ eq 5.74E-02 0 3.54E-05 0 3.72E-04 0
Eutrophication potential aquatic freshwater (EP-freshwater) kg P eq 1.29E-04 0 1.33E-09 0 8.9E-08 0
Eutrophication potential aquatic marine (EP-marine) kg N eq 1.41E-02 0 1.61E-05 0 9.52E-05 0
Eutrophication potential terrestrial (EP-terrestrial) mol N eq 1.5E-01 0 1.76E-04 0 1.05E-03 0
Formation potential of tropospheric ozone photochemical oxidants kg NMVOC
4.09E-02 0 3.2E-05 0 2.89E-04 0
(POCP) eq
Abiotic depletion potential for non fossil resources (ADPE) kg Sb eq 2.63E-04 0 4.28E-10 0 5.38E-09 0
Abiotic depletion potential for fossil resources (ADPF) MJ 2.79E+02 0 1.46E-01 0 6.88E-01 0
m3 world eq
Water use (WDP) 5.29E+00 0 8.99E-05 0 5.76E-03 0
deprived
RESULTS OF THE LCA - INDICATORS TO DESCRIBE RESOURCE USE according to EN 15804+A2: 1 m² Classic Lite ceiling
tiles (3.52 kg/m²)
Parameter Unit A1-A3 C1 C2 C3 C4 D
Renewable primary energy as energy carrier (PERE) MJ 1.05E+02 0 7.9E-04 0 1.03E-01 0
Renewable primary energy resources as material utilization
MJ 8.29E+00 0 0 0 0 0
(PERM)
Total use of renewable primary energy resources (PERT) MJ 1.13E+02 0 7.9E-04 0 1.03E-01 0
Non renewable primary energy as energy carrier (PENRE) MJ 2.78E+02 0 1.46E-01 0 6.89E-01 0
Non renewable primary energy as material utilization (PENRM) MJ 3.91E-01 0 0 0 0 0
Total use of non renewable primary energy resources (PENRT) MJ 2.79E+02 0 1.46E-01 0 6.89E-01 0
Use of secondary material (SM) kg 1.37E-01 0 0 0 0 0
Use of renewable secondary fuels (RSF) MJ 0 0 0 0 0 0
Use of non renewable secondary fuels (NRSF) MJ 0 0 0 0 0 0
Use of net fresh water (FW) m3 1.78E-01 0 2.27E-06 0 1.75E-04 0
RESULTS OF THE LCA – WASTE CATEGORIES AND OUTPUT FLOWS according to EN 15804+A2:
1 m² Classic Lite ceiling tiles (3.52 kg/m²)
Parameter Unit A1-A3 C1 C2 C3 C4 D
Hazardous waste disposed (HWD) kg 2.36E-06 0 3.66E-13 0 3.54E-11 0
Non hazardous waste disposed (NHWD) kg 3.31E+00 0 6.06E-06 0 3.52E+00 0
Radioactive waste disposed (RWD) kg 1.12E-02 0 8.22E-08 0 7.65E-06 0
Components for re-use (CRU) kg 0 0 0 0 0 0
Materials for recycling (MFR) kg 0 0 0 0 0 0
Materials for energy recovery (MER) kg 0 0 0 0 0 0
Exported electrical energy (EEE) MJ 0 0 0 0 0 0
Exported thermal energy (EET) MJ 0 0 0 0 0 0
RESULTS OF THE LCA – additional impact categories according to EN 15804+A2-optional:
1 m² Classic Lite ceiling tiles (3.52 kg/m²)
Parameter Unit A1-A3 C1 C2 C3 C4 D
Incidence of disease due to PM emissions (PM) Disease 5.86E-07 0 1.91E-10 0 4.58E-09 0
5 Environmental Product Declaration - Knauf Ceiling Solutions GmbH & Co. KG - Classic Lite
incidence
Human exposure efficiency relative to U235 (IR) kBq U235 eq 1.83E+00 0 5.45E-06 0 8.49E-04 0
Comparative toxic unit for ecosystems (ETP-fw) CTUe 8.92E+01 0 1.73E-01 0 3.85E-01 0
Comparative toxic unit for humans (carcinogenic) (HTP-c) CTUh 7.12E-08 0 2.78E-12 0 5.88E-11 0
Comparative toxic unit for humans (noncarcinogenic) (HTP-nc) CTUh 8.07E-06 0 9.62E-11 0 6.52E-09 0
Soil quality index (SQP) SQP 4.47E+02 0 4.31E-04 0 1.43E-01 0
Disclaimer 1 – for the indicator 'Potential Human exposure efficiency relative to U235'.
This impact category deals mainly with the eventual impact of low-dose ionizing radiation on human health of the nuclear fuel cycle. It
does not consider effects due to possible nuclear accidents, occupational exposure or radioactive waste disposal in underground
facilities. Potential ionizing radiation from the soil, radon and from some construction materials is also not measured by this indicator.
Disclaimer 2 – for the indicators 'abiotic depletion potential for non-fossil resources', 'abiotic depletion potential for fossil resources',
'water (user) deprivation potential, deprivation-weighted water consumption', 'potential comparative toxic unit for ecosystems', 'potential
comparative toxic unit for humans – cancerogenic', 'Potential comparative toxic unit for humans - not cancerogenic', 'potential soil
quality index'.
The results of this environmental impact indicator shall be used with care as the uncertainties on these results are high as there is
limited experience with the indicator.
6. LCA: Interpretation
The following interpretation contains a summary of the LCA mineral ceiling tiles.
results referenced to a declared unit of 1 m² Classic Lite
The comparison of the product's life cycle phases shows a role in all categories.
clear dominance of the production phase (modules A1–A3) in
all environmental impact categories. The potential The results of Classic Lite and Fine Fissured are identical.
environmental impacts from transport to disposal (module C2) Product specific results for Dune based on the results of
and the End of Life of the products due to landfilling (module Classic Lite are overestimated by about 3 % in all
C4) have a minor contribution. environmental impact categories.
The upstream supply chain of the raw board plays a dominant
7. Requisite evidence
7.1 Radioactivity biosoluble.
Not applicable for these products. Measuring point: Fraunhofer Institute for Toxicology and
Experimental Medicine
7.2 Biopersistence Certificate number: 02G15015 (5 September 2016)
The mineral wool used for the production of the panels is Test substance: Slag Wool 'Arm SW15'
6 Environmental Product Declaration - Knauf Ceiling Solutions GmbH & Co. KG - Classic Lite
7.3 VOC emissions Testing periode: 8.04.2020-28.04.2020
Measuring point: Central Chemical Lab of Intertek Testing Test basis: ASTM D5116-17
Services Ltd., Wuxi
Test report: Small-Scale Environmental Chamber Name Value Unit
Determinations of Organic Emissions From Indoor
TVOC < 0,02 mg/m³
Materials/Products
Formaldehyde emission <0,1 mg/m³
Number: 200408003SHF-001-R2
8. References
Standards and procedures.
ASTM C423-01 ISO 14044
ASTM C423-01:2001-07, Standard Test Method for Sound DIN EN ISO 14044:2006-10, Environmental management – Life
Absorption and Sound Absorption Coefficients by the cycle assessment – Requirements and guidelines.
Reverberation Room Method.
ISO 45001
ASTM E1414 DIN ISO 45001:2018-06, Occupational health and safety
ASTM E1414/E1414M-21a, Standard Test Method for Airborne management systems – Requirements with guidance for use.
Sound Attenuation Between Rooms Sharing a Common Ceiling
Plenum.
Further References
ASTM D5116-17
ASTM D5116-17, Small-Scale Environmental Chamber AVV, German List of Wastes Ordinance
Determinations of Organic Emissions from Indoor Regulation on the European Waste List. Waste Catalogue
Materials/Products. Ordinance (German designation: Abfallverzeichnisverordnung –
AVV) of 10 December 2001 (Federal Law Gazette I p. 3379),
ASTM E84 last amended by Article 1 of the Ordinance of 30 June 2020
ASTM E84, Standard Test Method for Surface Burning (Federal Law Gazette I p. 3005).
Characteristics of Building Materials.
Chemicals Prohibition Ordinance
ASTM E1414 Chemicals Prohibition Ordinance (German designation:
ASTM E1414/E1414M-21a, Standard Test Method for Airborne Chemikalien-Verbotsverordnung – ChemVerbotsV) of 20
Sound Attenuation Between Rooms Sharing a Common Ceiling January 2017 (Federal Law Gazette I p. 94; 2018 I p. 1389),
Plenum. last amended by Article 300 of the Ordinance of 19 June 2020
(Federal Law Gazette I p. 1328).
BS 476
BS 476-6:1989+A1:2009. Fire tests on building materials and ECHA-candidate list
structures. Method of test for fire propagation for products. List of substances of very high concern (SVHC) for
BS 476-7:1997. Fire tests on building materials and structures. authorisation (ECHA Candidate List), 25.06.2020, published
Method of test to determine the classification of the surface under Article 59(10) of REACH. Helsinki: European Chemicals
spread of flame of products. Agency.
EN 15804 Fraunhofer Institute for Toxicology and Experimental
DIN EN 15804:2012+A2:2019+AC:2021, Sustainability of Medicine
construction works – Environmental product declarations – Certificate number: 02G15015 (5 September 2016); Test
Core rules for the product category of construction products. substance: Slag Wool 'Arm SW15'.
ISO 354 GaBi
DIN EN ISO 354:2003-12, Acoustics – Measurement of sound GaBi 10, Software-System and Database for Life Cycle
absorption in reverberant rooms. Engineering. DB 2022.2. Sphera, 1992–2022. Available at:
https://gabi.sphera.com/support/gabi/
ISO 9001
DIN EN ISO 9001:2015-11, Quality management systems – IBU 2021
Requirements. Institut Bauen und Umwelt e.V.: General instructions for the
EPD programme of Institut Bauen und Umwelt e.V. (IBU).
ISO 10848 Version 2.0, Berlin: Institut Bauen und Umwelt e.V., 2021.
DIN EN ISO 10848-2:2006-08, Acoustics – Measurement of www.ibuepd.com
airborne and impact sound transmission between adjacent
rooms in test stands – Part 2: Application to lightweight Intertek Testing Services
components where the connection has a minor influence. Intertek Testing Services Shenzhen Ltd. Shanghai Fengxian
Branch; Test report: Small-Scale Environmental Chamber
ISO 14001 Determinations of Organic Emissions From Indoor
DIN EN ISO 14001:2015-11, Environmental management Materials/Products
systems – Requirements with guidance for use. Numbers: 200408003SHF-001-R2
ISO 14025 Ordinance on Biocide Products
DIN EN ISO 14025:2011-10, Environmental labels and Regulation (EU) No 528/2012 of the European Parliament and
declarations – Type III environmental declarations – Principles of the Council of 22 May 2012 concerning the making available
7 Environmental Product Declaration - Knauf Ceiling Solutions GmbH & Co. KG - Classic Lite
on the market and use of biocidal products. Umwelt e.V. (Hrsg.), 2022.
Ordinance on Hazardous Substances PCR: Mineral panels
Ordinance on Hazardous Substances, of 26 November 2010 Institut Bauen und Umwelt e.V. (IBU), 2023. Product Category
(Federal Law Gazette I p. 1643, 1644), last amended by Article Rules for Building-Related Products and Services. Part B:
148 of the Law of 29 March 2017 (Federal Law Gazette I p. Requirements on the EPD for Mineral panels. Version v2,
626). 31.05.2023.
PCR Part A REACH
Product category rules for building-related products and Regulation (EC) No 1907/2006 of the European Parliament and
services. Part A: Calculation rules for the life cycle assessment Council from 18 December 2006, Regulation concerning the
and requirements on the project report according to Registration, Evaluation, Authorisation and Restriction of
EN15804+A2:2019. Version 1.3, Berlin: Institut Bauen und Chemicals (REACH).
8 Environmental Product Declaration - Knauf Ceiling Solutions GmbH & Co. KG - Classic Lite
Publisher
Institut Bauen und Umwelt e.V. +49 (0)30 3087748- 0
Hegelplatz 1 info@ibu-epd.com
10117 Berlin www.ibu-epd.com
Germany
Programme holder
Institut Bauen und Umwelt e.V. +49 (0)30 3087748- 0
Hegelplatz 1 info@ibu-epd.com
10117 Berlin www.ibu-epd.com
Germany
Author of the Life Cycle Assessment
Daxner & Merl GmbH +43 676 849477826
Lindengasse 39/8 office@daxner-merl.com
1070 Wien www.daxner-merl.com
Austria
Owner of the Declaration
Knauf Ceiling Solutions GmbH & Co. KG 0049 8552 422 0
Elsenthal 15 info@knaufamf.com
94481 Grafenau www.knaufceilingsolutions.com
Germany
9 Environmental Product Declaration - Knauf Ceiling Solutions GmbH & Co. KG - Classic Lite
