ENVIRONMENTAL PRODUCT DECLARATION
as per ISO 14025 and EN 15804+A2
Owner of the Declaration Decospan NV
Publisher Institut Bauen und Umwelt e.V. (IBU)
Programme holder Institut Bauen und Umwelt e.V. (IBU)
Declaration number EPD-DEC-20230148-IBA1-EN
Issue date 29/08/2023
Valid to 28/08/2028
Veneered, wood flooring with HDF carrier (10 mm)
Decospan NV
www.ibu-epd.com | https://epd-online.com
1. General Information
Decospan NV Veneered, wood flooring with HDF carrier (10 mm)
Programme holder Owner of the declaration
IBU – Institut Bauen und Umwelt e.V. Decospan NV
Hegelplatz 1 Lageweg 33
10117 Berlin 8930 Menen
Germany Belgium
Declaration number Declared product / declared unit
EPD-DEC-20230148-IBA1-EN 1 m² of veneered, wood flooring with HDF carrier (10 mm)
This declaration is based on the product category rules: Scope:
Solid wood products, 01/08/2021 This Environmental Product Declaration covers an average square meter
(PCR checked and approved by the SVR) of pre-lacquered, veneered, wood flooring with HDF carrier (10 mm),
produced by Decospan NV in Belgium.
The owner of the declaration shall be liable for the underlying information
Issue date and evidence; the IBU shall not be liable with respect to manufacturer
information, life cycle assessment data and evidences.
29/08/2023
The EPD was created according to the specifications of EN 15804+A2. In
the following, the standard will be simplified as EN 15804.
Valid to
28/08/2028 Verification
The standard EN 15804 serves as the core PCR
Independent verification of the declaration and data according to ISO
14025:2011
internally X externally
Dipl.-Ing. Hans Peters
(Chairman of Institut Bauen und Umwelt e.V.)
Florian Pronold Dr. Matthew Fishwick,
(Managing Director Institut Bauen und Umwelt e.V.) (Independent verifier)
1 Environmental-Product Declaration - Decospan NV - Veneered, wood flooring with HDF carrier (10 mm)
2. Product
Constructional data
2.1 Product description/Product definition
Parky is a multi-layered parquet, consisting of a wood wear Name Value Unit
layer, pressed onto high-density fibreboard (HDF) with a Moisture content acc. to EN 322 5-9 %
wooden backing. Parky floors are finished with a top layer of Mean density 850 kg/m³
authentic wood species, sourced from responsible forestry. The
Thickness 10 mm
thickness of the veneer top layer is 0.6 mm in order to make the
Length 593 - 2050 mm
most of the material.
Width 121 - 233 mm
The thin veneer layer of 0.6 mm is pressed on the HDF board Reaction to fire EN 13501-1 Cfl-s1 Class
according to the DSI (Double-Sided Impregnation) system. Formaldehyde emission EN 717-1 E1 Class
During this process, the adhesive is pressed into and absorbed Content PCP EN 14342 < 5 ppm
by the wood.
Slip resistance CEN/TS 15676 ≥ 45 USRV
Thermal conductivity EN 12667 0.14 W/mK
The surface finish, consisting of eight robust layers of specially
developed lacquers protects the floor from wear and tear as Installation method floating -
well as scratches. The wood absorbs the varnish which fuses
Performance data of the product in accordance with the
with the adhesive. This results in a high-strength and scratch-
declaration of performance with respect to its essential
resistant floor and a moist and dirt-resistant surface.
characteristics according to EN 14342:2013, Wood flooring and
parquet - Characteristics, evaluation of conformity and marking.
The combination of the thin top layer, the high-densitiy
Verification and assessment of constancy of performance are
fibreboard and the wooden backing ensures impact resistance
carried out according to system 3.
and dimensional stability. Parky floors are equipped with a click
system for easy installation. 2.4 Delivery status
All products are delivered in packaging units. The following
To cover the most important products in the Parky product information is specified on the box:
range, three different product groups are distinguished, based
• Finish
on the product composition. The environmental profile was
• Wood type
calculated for each product group.
• Box quantity [m²]
• Dimensions [mm]
Group 1: Pre-lacquered, veneered wood flooring with HDF
• Number of parquet planks [pcs]
carrier (7-9 mm)
Group 2: Pre-lacquered, veneered wood flooring with HDF
Group 3 includes parquet planks with various formats.
carrier and cork backing (10-12 mm)
Dimensions of the declared products as delivered are within
Group 3: Pre-lacquered, veneered wood flooring with HDF
following ranges:
carrier (10 mm)
• Length: 593 - 2050 mm
This EPD applies to Group 3: pre-lacquered, veneered flooring • Width: 121 - 233 mm
with HDF carrier (10 mm). • Thickness: 10 mm
• Box quantity: 0.79 -2.39 m²
For the placing on the market of the product in the European
2.5 Base materials/Ancillary materials
Union/European Free Trade Association (EU/EFTA) (with the
exception of Switzerland) Regulation (EU) No. 305/2011 (CPR) The average composition of the finished products is calculated
applies. The product needs a declaration of performance taking per product group. The components of group 3 are given below
into consideration EN 14342:2013 Wood flooring and parquet - in kg/m² flooring.
Characteristics, evaluation of conformity and marking as well as • Lacquer < 1.5 %
the CE-marking. Further specification is according to EN • Veneer (top layer & backing) 9 %
14354:2017, the European standard for wood veneer floor • Adhesive (UF-glue) < 1 %
coverings, as referenced by EN 14342:2013. For the • High-density fibreboard 89 %
application and use., the respective national provisions apply.
This product/article/at least one partial article contains
2.2 Application
substances listed in the candidate list (17.01.2023) exceeding
Parky flooring is covered by harmonised standards, EN 0.1 percentage by mass: No
14342:2013 and EN 14354:2017. It's intended as floor covering
for internal use in dry conditions. The provided click system is This product/article/at least one partial article contains other
only suitable for floating installations. Flooring without an carcinogenic, mutagenic, reprotoxic (CMR) substances in
integrated cork layer should be installed on a suitable underlay. categories 1A or 1B which are not on the candidate list,
Parky flooring can be installed for both private and commercial exceeding 0.1 percentage by mass: No
use. The installation must be carried out in accordance with the
installation instructions, the rules of the trade and the state of Biocide products were added to this construction product or it
the art. has been treated with biocide products (this then concerns a
treated product as defined by the (EU) Ordinance on Biocide
2.3 Technical Data
Products No. 528/2012): No
Technical specifications in accordance with the information in
the declaration of performance with respect to its essential 2.6 Manufacture
characteristics following EN 14342:2013, Wood flooring and Decospan produces Parky flooring at its production site in
parquet - Characteristics, evaluation of conformity and marking. Belgium. The production process mainly involves assembly of
2 Environmental-Product Declaration - Decospan NV - Veneered, wood flooring with HDF carrier (10 mm)
the above, purchased components (HDF, veneer, adhesive, Possible hazards, related to chemicals used in production, are
lacquer). Prior to the assembly process, an extended part of the covered by a yearly due diligence exercise where material
production is dedicated to the sorting, preparing and jointing of safety data sheets are collected and conformity with the
the veneer. REACH-regulation (incl. SVHC's) is evaluated.
Veneer is produced by slicing a log into thin layers. This The health and safety manager keeps track of safe use
process makes optimal use of the logs because, in contrast guidelines and provides appropriate personal protection
with solid wood, there is no sawing loss. Since Decospan equipment when needed. Since air extraction systems filter
purchases bundles of sliced veneer, the production process in ambient air in production, personal protection equipment mainly
Belgium starts with a sorting process. involves:
Incoming veneer bundles are evaluated on various aspects:
• Protective clothing
• Wood species • Safety shoes
• Slicing technique • Hearing protection
• Dimensions • Gloves
• Quality All employees are provided with the above mentioned, suitable
After the assignment of a certain quality level, the bundles are protection measures.
cut in length and width. By using advanced technology, the
sliced wood can be joined into veneer sheets, which are again A committee for prevention and protection at work is in place.
graded, based on their quality. Training for personnel is carried out at regular intervals,
including: at the start of employment, annual recap or when
The next step in the production process is pressing. Adhesive is deemed necessary.
applied to both sides of the HDF carrier, which is subsequently All of this is captured in safety procedures, prevention and
placed onto the wooden backing. The wooden wear layer is protection reports and put into practice by means of e.g. fire
placed on top. By placing this combination of materials in the exercises, first aid training organized by the HR- and HSE-
press at a predefined time, temperature and pressure level, the manager.
adhesive is pressed into and absorbed by the wood. After
pressing, the veneered board is trimmed to the desired Chemical residues are sorted and collected separately. These
dimensions and subjected to quality control. containers are picked up by our waste processor and
processed according to applicable disposal regulations.
Finishing of the wooden wear layer is done by applying eight
layers of specially developed lacquers. Prior to this process, the Environmental protection measures:
wooden wear layer is sanded and optionally brushed. The eight Decospan is FSC® (FSC-C095327) and Program for the
layers of lacquer are cured by means of UV light. This Enforcement of Forest Certification (PEFC) certified. Both
extremely strong and matt lacquer is nearly invisible. The organisations are committed to responsible forest management
quality of the finishing process is extensively inspected. and include social aspects in their policy. Wood or wood-based
materials are responsibly sourced with one of the above-
After approval of the finishing quality, the lacquered veneered mentioned certifications or as 'Pure Wood'. All suppliers are
boards are divided into parquet planks. Dimensions of the requested to sign and comply with the Pure Wood charter and
planks depend on the collection. Each plank is provided with a thus respect and commit to Decospans core values concerning
click system, which is carefully milled to the sides. responsible forestry.
Internal wood waste is incinerated with energy recovery which
The wooden flooring is packed in cardboard boxes and is re-used in the manufacturing process. Air extraction systems
wrapped with plastic foil. filter ambient air in production. A committee for prevention and
protection at work is in place.
At the end of the manufacturing process, a full quality
inspection check is performed and documented according to 2.8 Product processing/Installation
the internal Factory Production Control (FPC) system. Before starting the installation, it is essential to read the Parky
installation instructions carefully. Parky flooring is intended for
floating installation and can easily be installed, with its click
tongue-and-groove system. Following installation tools are
recommended:
• Parky installation kit
• Pencil
• Meter
• Hammer
• Handsaw
• Cutter
Besides the above-mentioned installation tools, Parky flooring
can be processed with all tools, suitable for solid wood. These
tools must be operated in accordance with the manufacturer's
operating instructions. Make sure that the necessary safety
precautions and protection measures (e.g. hearing protection,
2.7 Environment and health during manufacturing respiratory mask, protective gloves, safety glasses...) are
Health protection measures applied. Provide adequate ventilation if the processing
Decospan strictly and fully applies applicable legislation and operations generate wood dust.
also complies with all requirements for general good working
conditions, in particular, with regard to health and safety. Dispose of the product and packaging in accordance with
applicable, local, or national disposal regulations.
3 Environmental-Product Declaration - Decospan NV - Veneered, wood flooring with HDF carrier (10 mm)
life. This also applies for unusually low or high humidity,
2.9 Packaging excessive water use, dragging heavy furniture, etc.
Parky flooring is packed in a cardboard box and wrapped with Description of the influences on the ageing of the product when
PE-foil in order to protect the product during transport and applied in accordance with the rules of technology.
storage.
Packaging material must be collected separately and disposed
of in accordance with applicable legislation. 2.13 Extraordinary effects
Fire
2.10 Condition of use Parky, wood veneered floor covering, with surface coating and
Before installation, Parky flooring should be stored in a dry and with or without cork bottom layer is classified as Cfl-s1. Test
protected room with an air humidity of 40 – 60 % and a conditions: in accordance with EN 13501-1:2019 . Installation
temperature between 16-21°C. Wood has, as a hygroscopic method: loose-laid on end-use substrates of wood and of
material, the ability to absorb and release moisture from the classes A1 and A2-s1,d0.
surrounding environment. Changes in moisture content can
Fire protection
result in dimensional changes over time. This needs to be
accommodated during installation by foreseeing expansion Name Value
gaps of 1 mm per running meter, as outlined in the installation Building material class Cfl
instructions. Smoke gas development s1
2.11 Environment and health during use
Water
The use phase of Parky flooring is not in the scope of the Life
Parky flooring has a water-resistant surface but is not able to
Cycle Assessment (LCA) and resulting EPD. However,
withstand prolonged exposure to water. Besides damage to the
measurements of VOC emissions to indoor air are measured
product, no adverse consequences to the environment will
and available.
occur.
Parky flooring complies with following regulations and test
Mechanical destruction
protocols:
No negative impacts on the environment are identified when
• Indoor Air Comfort GOLD®
mechanically destroying the product. Suitable personal
• CDPH
protection equipment is recommended to prevent injury or
• M1
health risks, caused by sharp edges, wood chips or wood dust.
Additional and more detailed information can be provided on
request. Parky flooring does not imply any hazards to water, air 2.14 Re-use phase
or soil when used as intended. Limited mechanical damage like scratches can be repaired
using the Parky Repair Pens and Parky Repair Wax. Colour
2.12 Reference service life
and lacquer pens are available to repair the floor and to protect
The service life in accordance with the Bundsinstitut fûr Stadt-
it from dirt and moisture.
und Raumforschung (BBSR), table "Service lives of
components for life cycle assessment according to
When your floor is severely damaged, the Parky Bulldog allows
Bewertungssystem Nachhaltiges Bauen (BNB)", is
you to remove and replace the damaged plank(s). More
• 40 years for wooden, multilayer parquet. information and instructions for use are available on www.par-
• 15 years for wood lacquers ky-com.
The service life is specified on an informative basis and is
based on the warranty period Decospan specifies for the At end-of-life, the product can be incinerated with energy
products: recovery.
2.15 Disposal
Parky flooring is classified as wood waste with EWC-code 17
02 01, according to EUROSTAT Guidance.
The product must be disposed of in accordance with applicable,
local or national disposal regulations.
The following information, related to maintenance and repair is 2.16 Further information
informative, given that module B is not declared. The product
Additional information, contact details, installation and
must be installed and maintained according to the Parky
maintenance instructions are available on www.par-ky.com
installation and maintenance instructions.
Misuse or poor maintenance will adversely affect the service
3. LCA: Calculation rules
largest since the amount of HDF can vary +/- 11 %. For group 1
3.1 Declared Unit and 3 these differences are smaller, respectively 3.82 % and
The declared unit is 1 m² of pre-lacquered, veneered wood 5.88 %.
flooring with HDF carrier of 10 mm. The total inputs, outputs
Declared unit
and produced m² for the period under consideration are taken
as a basis.
The products in this EPD represent an average in a product
group. The most important variable which leads to differences
in the environmental profiles within the group is the amount of
HDF in these products. In group 2 these differences are the
4 Environmental-Product Declaration - Decospan NV - Veneered, wood flooring with HDF carrier (10 mm)
Name Value Unit
Final waste treatment C4
Declared unit 1 m²
The waste treatment scenario in this study assumes that that
Gross density 850 kg/m3
the wood chips are used for incineration with energy recovery.
Grammage 9.49 kg/m2
3.4 Cut-off criteria
Wood moisture at delivery 5 - 9 %
Emissions for the combustion of wood are not measured at the
Weighted averged thickness 10 mm
plant and are therefore included via the ecoinvent used. There
Decospan collected data for a full production year: 2021. More is a process-specific emission to be expected from
specifically: formaldehyde. The exact emission is not measured and
• Raw material use and transport to the production therefore included based on the ecoinvent process "Glued
location laminated timber, for indoor use {RER}| production | Cut-off".
• Decospan contacted relevant suppliers for primary data The emission included in the calculation is 0.0114 kg/m3
• Energy use product. The avoided production of electricity from primary
• Emissions sources is based on: "Electricity, high voltage {NL}|heat and
• Production power co-generation, natural gas, combined cycle power plant,
400MWelectrical | Cut-off". The avoided production of heat from
3.2 System boundary primary sources is based on: "Heat, district or industrial, natural
This EPD is a cradle-to-gate with options (C1-C4, D) gas {Europe without Switzerland}| heat production, natural gas,
at industrial furnace >100 kW |Cut-off".
Product stage A1-A3
Parquet consists of a high-density fibreboard to which a Since the LCA is based on production information from a full
wooden veneer layer is applied (glued) on both sides. All the production year it is expected that mass and energy balance is
raw materials are supplied to Decospan by truck. The (in) close (proximity) to complete as no materials or processes
application of veneer onto the baseboard is called the pressing have been excluded. The cut-off criteria are well below 1 %.
process. This pressing is achieved by means of pressure,
3.5 Background data
temperature and time. The panels are then sawn, sanded and
varnished. After varnishing, the boards are divided in planks For background processes, the ecoinvent database v3.6
and are provided with a click system so that they can be clipped (allocation cut-off) has been used.
into one another.
3.6 Data quality
Data quality and validation of economic flows
The heat used in the production process is obtained from the
Decospan collected data on the production of Parky parquet for
incineration of part of Decospan's wood production waste.
a full production year, 2021. More
specifically:
The proportion of the electricity demand covered by green
electricity in the total electricity demand is 100 %. • Raw material use and transport to the production
location
Transport to construction (A4) • Primary data for important products were requested
This module is not in the scope of this EPD. from suppliers
• Energy use
Construction process (A5) • Emissions
This module is not in the scope of this EPD. • Production waste
Use phase (B) The provided data was checked for plausibility. The quality and
This module is not in the scope of this EPD. However, the representativeness are considered high. The products in this
emissions to indoor air will be mentioned informatively in this EPD represent an average in a product group. The most
EPD. important variable which leads to differences in the
environmental profiles within the group is the amount of HDF in
Demolition C1 these products. In group 2 these differences are the largest
Parquet can be removed from the building in a manual process. since the amount of HDF can vary +/- 11 %. For group 1 and 3
It is anticipated that the environmental impact of this process is these differences are smaller, respectively 3.82 % and 5.88 %.
neglectable.
For background processes, the ecoinvent database v3.6
Recovery D (allocation cut-off) has been used.
This module includes the benefit of the recovery of electricity
and heat that often occurs in waste incineration plants. For the Data quality and validation of environmental inventories
electrical and thermal efficiency of the waste-to-energy plant we Since the LCA is based on production information from a full
calculated with 18 % and 31 % respectively. For the heat of production year it is expected that mass and energy balance is
combustion of parquet (wood) the lower heating value was close to complete. For the LCA calculations, the following
used: Wood: 13.99 MJ/kg. methods have been used:
• SimaPro's LCA method: "EN 15804+A2" via
3.3 Estimates and assumptions
bepalingsmethode 'set 1', 'set 2' & param (NMD 3.4)
Transport to waste treatment C2
(see appendix C)
After the parquet is removed from the application is transported
SGS INSTRON has checked potential uncharacterised
to a waste treatment facility. In the waste treatment scenario in
substances. This check is part of the validation of
this LCA, a transport distance of 50 km is assumed.
environmental inventories.
Waste processing C3 3.7 Period under review
The waste treatment scenario in this study assumes that at the
The production data for this EPD is based on the production of
waste treatment facility the parquet is chipped into wood chips.
a full production year (2021).
5 Environmental-Product Declaration - Decospan NV - Veneered, wood flooring with HDF carrier (10 mm)
the mass of the products and the loss factor for each of the
3.8 Geographic Representativeness products.
Land or region, in which the declared product system is
manufactured, used or handled at the end of the product´s 3.10 Comparability
lifespan: Belgium Basically, a comparison or an evaluation of EPD data is only
possible if all the data sets to be compared were created
according to EN 15804 and the building context, respectively
3.9 Allocation
the product-specific characteristics of performance, are taken
The energy use for the production processes has been into account. For background processes, the ecoinvent
allocated based on the area produced for each of the products. database v3.6 (allocation cut-off) has been used.
The amount of production waste has been allocated based on
4. LCA: Scenarios and additional technical information
The service life is declared in accordance with the BBSR, table
Characteristic product properties biogenic carbon "Service lives of components for life cycle assessment
The amount of biogenic C in the product has been calculated according to BNB".
using the amount of veneer, HDF and cork in the product,
Name Value Unit
multiplication by the wood and cardboard content and 0.5. The
Life span according to BBSR 15 years
latter is the amount of C in wood according to EN 16485:2014.
The wood content in HDF is 77 % according to the suppliers Life span according to the See section -
EPD: EPD-UNI-20150013-IBA1-EN. For veneer and cork, a manufacturer 2.12
moisture content of 6 % has been used.
End of life (C1-C4)
Note: 1 kg of biogenic carbon is equivalent to 44/12 kg of CO .
2
Information on describing the biogenic carbon content at Demolition C1
factory gate Parquet is typically removed from the building in a manual
Name ValueUnit process. It is anticipated that the environmental impact of this
kg process is neglectable.
Biogenic carbon content in product 3.67
C
Transport to waste treatment C2
Biogenic carbon content in accompanying kg
0.08 After the parquet is removed from the application it's
packaging C
transported to a waste treatment facility. In the waste treatment
scenario in this LCA a transport distance of 50 km is assumed
Use or application of the installed product (B1) see (ecoinvent: "Transport, freight, lorry, unspecified {GLO}| market
section 2.12 "Use" group for transport, freight, lorry, unspecified | Cut-off)".
This module is not in scope. However, the emissions to indoor
air are informatively mentioned in section 2.11. Waste processing (C3)
The waste treatment scenario in this study assumes that at the
The following information, related to maintenance and repair is waste treatment facility the parquet is chipped into wood chips.
informative, given that module B is not declared. The following ecoinvent process is used: "Wood chipping,
industrial residual wood, stationary electric chipper {GLO}|
Maintenance (B2) market for | Cut-off".
The specially developed Parky Wood Floor Cleaner is
recommended to maintain the parquet. It removes dirt without Final waste treatment (C4)
harming the lacquer. Maintenance instructions are available on The waste treatment scenario in this study assumes that the
www.par-ky.com wood chips are used for incineration with energy recovery. It is
assumed that the energy efficiency of energy recovery is 18 %
Repair (B3) electric and 31 % thermal. Since this efficiency is <60 %, the
Limited mechanical damage like scratches can be repaired incineration process is included in module C4.
using the Parky Repair Pens and Parky Repair Wax. Colour
Name Value Unit
and lacquer pens are available to repair the floor and protect it
Collected separately waste wood 9.49 kg
from dirt and moisture.
Energy recovery 9.49 kg
Replacement (B4) / Refurbishment (B5)
When your floor is severely damaged, the Parky Bulldog allows Reuse, recovery and/or recycling potentials (D), relevant
you to remove and replace the damaged plank(s). More scenario information.
information and instructions for use are available on www.par- The benefit of the recuperation of electricity and heat that often
ky-com. occurs in waste incineration plants was included in module D.
Reference service life
6 Environmental-Product Declaration - Decospan NV - Veneered, wood flooring with HDF carrier (10 mm)
5. LCA: Results
DESCRIPTION OF THE SYSTEM BOUNDARY (X = INCLUDED IN LCA; ND = MODULE OR INDICATOR NOT DECLARED; MNR =
MODULE NOT RELEVANT)
Benefits and
Construction loads beyond
Product stage Use stage End of life stage
process stage the system
boundaries
la ire ta m w a Ry lp p u s tro p s n a rT g n iru tc a fu n a M e h t m o rf tro p s n a rTe tis e h t o t e ta g y lb m e s s A e s U e c n a n e tn ia M ria p e R tn e m e c a lp e R tn e m h s ib ru fe R y g re n e la n o ita re p Oe s u re ta w la n o ita re p Oe s u n o itc u rts n o c -e Dn o itilo m e d tro p s n a rT g n is s e c o rp e ts a W la s o p s iD -e s u e R-y re v o c e R-g n ilc y c e Rla itn e to p
A1 A2 A3 A4 A5 B1 B2 B3 B4 B5 B6 B7 C1 C2 C3 C4 D
X X X MND MND MND MND MNR MNR MNR MND MND X X X X X
RESULTS OF THE LCA - ENVIRONMENTAL IMPACT according to EN 15804+A2: 1 m2 veneered wood flooring with HDF carrier
(10 mm)
Parameter Unit A1-A3 C1 C2 C3 C4 D
Global Warming Potential total (GWP-total) kg CO 2 eq -3.7E+00 0 1.32E-01 1.34E-01 1.7E+01 -6.35E-01
Global Warming Potential fossil fuels (GWP-fossil) kg CO 2 eq 1.29E+01 0 1.32E-01 1.33E-01 1.42E-01 -5.69E-01
Global Warming Potential biogenic (GWP-biogenic) kg CO 2 eq -1.68E+01 0 6.07E-05 1.04E-03 1.68E+01 -5.88E-02
Global Warming Potential luluc (GWP-luluc) kg CO 2 eq 1.9E-01 0 4.82E-05 2.39E-04 2.53E-05 -6.55E-03
Depletion potential of the stratospheric ozone layer (ODP) kg CFC11 eq 8.55E-07 0 2.9E-08 6.03E-09 1.14E-08 -1.67E-07
Acidification potential of land and water (AP) mol H+ eq 9.03E-02 0 7.63E-04 6.75E-04 1.6E-03 -1.85E-02
Eutrophication potential aquatic freshwater (EP-freshwater) kg P eq 1.9E-03 0 1.33E-06 8.1E-06 1.85E-06 -5.84E-05
Eutrophication potential aquatic marine (EP-marine) kg N eq 1.59E-02 0 2.69E-04 1.12E-04 7.54E-04 -5.42E-03
Eutrophication potential terrestrial (EP-terrestrial) mol N eq 1.79E-01 0 2.96E-03 1.28E-03 8.03E-03 -8.92E-02
Formation potential of tropospheric ozone photochemical oxidants kg NMVOC
6E-02 0 8.46E-04 3.44E-04 1.98E-03 -1.56E-02
(POCP) eq
Abiotic depletion potential for non fossil resources (ADPE) kg Sb eq 1.05E-04 0 3.33E-06 3.27E-07 1.83E-06 -8.37E-06
Abiotic depletion potential for fossil resources (ADPF) MJ 1.92E+02 0 1.98E+00 1.82E+00 1.24E+00 -6.84E+00
m3 world eq
Water use (WDP) 3.5E+00 0 7.1E-03 2.22E-02 -1.1E-01 -6.1E-02
deprived
RESULTS OF THE LCA - INDICATORS TO DESCRIBE RESOURCE USE according to EN 15804+A2: 1 m2 veneered wood
flooring with HDF carrier (10 mm)
Parameter Unit A1-A3 C1 C2 C3 C4 D
Renewable primary energy as energy carrier (PERE) MJ 2.86E+02 0 2.48E-02 2.23E-01 2.83E-02 -1.48E+02
Renewable primary energy resources as material utilization
MJ 0 0 0 0 0 0
(PERM)
Total use of renewable primary energy resources (PERT) MJ 2.86E+02 0 2.48E-02 2.23E-01 2.83E-02 -1.48E+02
Non renewable primary energy as energy carrier (PENRE) MJ 2.03E+02 0 2.11E+00 1.92E+00 1.35E+00 -7.27E+00
Non renewable primary energy as material utilization (PENRM) MJ 0 0 0 0 0 0
Total use of non renewable primary energy resources (PENRT) MJ 2.03E+02 0 2.11E+00 1.92E+00 1.35E+00 -7.27E+00
Use of secondary material (SM) kg 0 0 0 0 0 0
Use of renewable secondary fuels (RSF) MJ 0 0 0 0 0 0
Use of non renewable secondary fuels (NRSF) MJ 0 0 0 0 0 0
Use of net fresh water (FW) m3 1.2E-01 0 2.42E-04 1.08E-03 -2.07E-03 -1.82E-03
RESULTS OF THE LCA – WASTE CATEGORIES AND OUTPUT FLOWS according to EN 15804+A2:
1 m2 veneered wood flooring with HDF carrier (10 mm)
Parameter Unit A1-A3 C1 C2 C3 C4 D
Hazardous waste disposed (HWD) kg 2.3E-02 0 5.03E-06 7.44E-07 2.88E-06 -2.43E-05
Non hazardous waste disposed (NHWD) kg 2.23E+00 0 1.26E-01 1.22E-02 1.13E-01 -2.66E-01
Radioactive waste disposed (RWD) kg 8.31E-04 0 1.3E-05 7.01E-06 2.76E-06 -4.4E-05
Components for re-use (CRU) kg 0 0 0 0 0 0
Materials for recycling (MFR) kg 0 0 0 0 0 0
Materials for energy recovery (MER) kg 0 0 0 0 0 0
Exported electrical energy (EEE) MJ 0 0 0 0 2.45E+01 0
Exported thermal energy (EET) MJ 0 0 0 0 4.23E+01 0
RESULTS OF THE LCA – additional impact categories according to EN 15804+A2-optional:
1 m2 veneered wood flooring with HDF carrier (10 mm)
Parameter Unit A1-A3 C1 C2 C3 C4 D
Disease
Incidence of disease due to PM emissions (PM) 9.57E-07 0 1.18E-08 4.73E-09 1.66E-08 -2.51E-07
incidence
Human exposure efficiency relative to U235 (IR) kBq U235 eq 8.27E-01 0 8.31E-03 9.31E-03 2.04E-03 -2.87E-02
7 Environmental-Product Declaration - Decospan NV - Veneered, wood flooring with HDF carrier (10 mm)
Comparative toxic unit for ecosystems (ETP-fw) CTUe 3.58E+02 0 1.77E+00 2.37E+00 2.23E+00 -1.8E+02
Comparative toxic unit for humans (carcinogenic) (HTP-c) CTUh 2.28E-08 0 5.74E-11 4.83E-11 3.95E-10 -2.06E-09
Comparative toxic unit for humans (noncarcinogenic) (HTP-nc) CTUh 1.91E-07 0 1.93E-09 1.35E-09 2.1E-08 -7.51E-08
Soil quality index (SQP) SQP 1.48E+03 0 1.72E+00 3.27E-01 3.89E-01 -7.07E+02
Disclaimer 1 – for the indicator “Potential Human exposure efficiency relative to U235”. This impact category deals mainly with the
eventual impact of low-dose ionizing radiation on human health of the nuclear fuel cycle. It does not consider effects due to possible
nuclear accidents, occupational exposure nor due to radioactive waste disposal in underground facilities. Potential ionizing radiation
from the soil, from radon and from some construction materials is also not measured by this indicator.
Disclaimer 2 – for the indicators “abiotic depletion potential for non-fossil resources”, “abiotic depletion potential for fossil resources”,
“water (user) deprivation potential, deprivation-weighted water consumption”, “potential comparative toxic unit for ecosystems”,
“potential comparative toxic unit for humans – cancerogenic”, “Potential comparative toxic unit for humans - not cancerogenic”,
“potential soil quality index”. The results of this environmental impact indicator shall be used with care as the uncertainties on these
results are high or as there is limited experienced with the indicator.
6. LCA: Interpretation
parquet.
To visualize which materials and processes give the largest
contribution to the environmental indicators, a major The production of HDF gives the largest contribution to most of
contributions analysis has been included. In the graph, the total the environmental indicators. The exceptions are GWP where
value of each indicator has been set to 100 %. The colours the incineration of wood (waste) gives the largest contribution.
indicate which part of the environmental effects are caused by
the different materials and processes in the life cycle of the
7. Requisite evidence
Use phase (B) is not in the scope of this LCA, however, the Name Value Unit
emissions to indoor air will be mentioned informatively. VOC TVOC (C6 - C16) 6.1 μg/m3
emission test reports by Eurofins Product Testing A/S,
Sum SVOC (C16 - C22) < 5 μg/m3
Smedeskovvej 38, 8464 Galten, Denmark are available. The
highest measured values of all objects, included in group 3, is R (dimensionless) 0.092 -
given. VOC without NIK < 5 μg/m3
7.1. Formalehyde
Carcinogenic Substances < 1 μg/m3
Test method: EN 16516
Name Value Unit
EN 717-1 8.5 µg/m³
AgBB overview of results (3 days [µg/m³])
Name Value Unit
7.2. VOC emissions
TVOC (C6 - C16) 12 μg/m3
AgBB overview of results (28 days [µg/m³])
Sum SVOC (C16 - C22) < 5 μg/m3
R (dimensionless) 0.077 -
VOC without NIK < 5 μg/m3
Carcinogenic Substances < 1 μg/m3
8 Environmental-Product Declaration - Decospan NV - Veneered, wood flooring with HDF carrier (10 mm)
Name Value Unit
French VOC regulation A(+) -
Comparison with limit values of
French CMR components Pass -
- French VOC Regulation
Belgian Regulation Pass -
- French CMR Components
- Belgian Regulation
8. References
Standards ISO 21930:2017 Sustainability in buildings and civil engineering
works — Core rules for environmental product declarations of
EN 322 construction products and services, 2017.
EN 322:1994, Wood-based panels - Determination of moisture Further references
content
AgBB/ABG
EN 717-1 Anforderungen an bauliche Anlagen bezüglich des
EN 717-1:5802004, Wood-based panels - Determination of Gesundheitsschutzes (ABG)
formaldehyde release - Part 1: Formaldehyde emission by the
chamber method AltholzV
Ordinance on Requirements for the Recovery and Disposal of
EN 12667 Waste Wood of 15 August 2002 (BGBl. I p. 3302), last
EN 12667:2001, Thermal performance of building materials and amended by Article 120 of the Ordinance of 19 June 2020
products - Determination of thermal resistance by means of (BGBl. I p. 1328).
guarded hot plate and heat flow meter methods - Products of
high and medium thermal resistance Belgian Regulation
Royal decree of May 2015
EN 13501-1
EN 13501-1:2019, Fire classification of construction products BBSR
and building elements - Part 1: Classification using data from Bundesinstitut für Bau-, Stadt- und Raumforschung
reaction to fire tests
BNB
ISO 14025 BNB Code No. 352.812 Useful lives of building components for
ISO 14025:2006 Environmental labels and declarations — Type life cycle analyses according to the Sustainable Building
III environmental declarations — Principles and procedures, Assessment System, 2017: Wood multilayer parquet. Berlin:
2006. Federal Ministry of the Interior, for Construction and Home
Affairs.
ISO 14040
ISO 14040:2006 Environmental management — Life cycle CDPH
assessment — Principles and framework, 2006. Californian Department of Public Health Standard Method for
VOC Emissions
ISO 14044
ISO 14044:2006 Environmental management — Life cycle ECHA Candidate List
assessment — Requirements and guidelines, 2006. List of Substances of Very High Concern (SVHC) Candidate for
Authorisation (ECHA Candidate List), dated 17.01.2023,
EN 14342 published in accordance with Article 59(10) of the REACH
EN 14342:2013, Wood flooring - Characteristics, evaluation of Regulation. Helsinki: European Chemicals Agency.
conformity and marking
EUROSTAT
EN 14354 European waste classification for statistics
EN 14354: 2017, Wood veneer floor coverings
EWC-code
CEN/TS 15676 EWC-code 17 02 01: Non-hazardous wood waste
CEN/TS 15676:2007, Wood flooring, slip resistance
French VOC Regulation
EN 15804 Regulation of March and May 2011 (DEVL1101903D and
EN 15804:2012+A2:2019, Sustainability of construction works - DEVL1104875A)
Environmental product declarations - Core rules for the product
category of construction products, 2019. French CMR Components
Regulation of April and May 2009
EN 16485
EN 16485:2014; Round and sawn timber - Environmental FSC®
Product Declarations - Product category rules for wood and Forest Stewardship Council License number: FSC-C095327
wood-based products for use in construction, 2014.
IBU 2021
EN 16516 Institut Bauen und Umwelt e.V.: General Instructions for the
EN 16516:2017+A1:2020, Construction products: Assessment EPD programme of Institut Bauen und Umwelt e.V., Version
of release of dangerous substances - Determination of 2.0, Berlin: Institut Bauen und Umwelt e.V., 2021 HYPERLINK
emissions into indoor air. "http://www.ibu-epd." www.ibu-epd.com
ISO 21930
9 Environmental-Product Declaration - Decospan NV - Veneered, wood flooring with HDF carrier (10 mm)
Indoor Air Comfort Gold® 'Product Category Rules for Building-Related Products and
Eurofins product certification Services Part B: Requirements on the EPD for Solid wood
products.'
M1 Institut Bauen und Umwelt e.V., 2021.
Finnish classification test for building materials
Regulation (EU) No 305/2011
PEFC of the European Parliament and of the Council of 9 March 2011
Programme for the Endorsement of Forest Certification laying down harmonised conditions for the marketing of
Schemes. construction products
License number: PEFC/07-31-60
Regulation (EU) No 528/2012
PCR Part A of the European Parliament and the Council of 12 May 2012
'Product Category Rules for Building-Related Products and concerning the making available on the market and use of
Services Part A: Calculation Rules for the Life Cycle biocidal products.
Assessment and Requirements on the Project Report according
to EN 15804+A2:2019 Version 1.3,' Software/database
Ecoinvent database v3.6
PCR Part B
10 Environmental-Product Declaration - Decospan NV - Veneered, wood flooring with HDF carrier (10 mm)
Publisher
Institut Bauen und Umwelt e.V. +49 (0)30 3087748- 0
Hegelplatz 1 info@ibu-epd.com
10117 Berlin www.ibu-epd.com
Germany
Programme holder
Institut Bauen und Umwelt e.V. +49 (0)30 3087748- 0
Hegelplatz 1 info@ibu-epd.com
10117 Berlin www.ibu-epd.com
Germany
Author of the Life Cycle Assessment
SGS INTRON +31 88 214 52 04
Dr. Nolenslaan 126 nl.intron@sgs.com
6136GV Sittard www.sgs.com/intron
Netherlands
Owner of the Declaration
Decospan NV +32 (0)56 88 99 00
Lageweg 33 compliance@decospan.com
8930 Menen https://www.decospan.com/
Belgium
11 Environmental-Product Declaration - Decospan NV - Veneered, wood flooring with HDF carrier (10 mm)
