ENVIRONMENTAL PRODUCT DECLARATION
as per ISO 14025 and EN 15804+A2
Owner of the Declaration Grundfos Holding A/S
Publisher Institut Bauen und Umwelt e.V. (IBU)
Programme holder Institut Bauen und Umwelt e.V. (IBU)
Declaration number EPD-GRU-20240017-CBA1-EN
Issue date 21.03.2024
Valid to 20.03.2029
MAGNA3 65-80/100/120 (Stainless Steel)
Grundfos Holding A/S
www.ibu-epd.com | https://epd-online.com
General Information
Grundfos Holding A/S MAGNA3 65-80/100/120 (Stainless Steel)
Programme holder Owner of the declaration
IBU – Institut Bauen und Umwelt e.V. Grundfos Holding A/S
Hegelplatz 1 Poul Due Jensens Vej 7
10117 Berlin 8850 Bjerringbro
Germany Denmark
Declaration number Declared product / declared unit
EPD-GRU-20240017-CBA1-EN 1 PCS. of MAGNA3 65-80/100/120 (Stainless Steel)
This declaration is based on the product category rules: Scope:
Pumps for liquids and liquids with solids, 01.08.2021 The declaration applies to 1 piece of MAGNA3 (Stainless Steel) pump.
(PCR checked and approved by the SVR)
Issue date The product is produced in Wahlstedt, Germany, and the life cycle
assessment is based on data collected at the production site.
21.03.2024
Valid to
Production has been modeled using annual production data from 2021.
20.03.2029
The declaration covers three different types of the MAGNA3 65- product
(80/100/120).
The owner of the declaration shall be liable for the underlying information
and evidence; the IBU shall not be liable with respect to manufacturer
information, life cycle assessment data and evidences.
The EPD was created according to the specifications of EN 15804+A2. In
the following, the standard will be simplified as EN 15804.
Verification
Dipl.-Ing. Hans Peters
(Chairman of Institut Bauen und Umwelt e.V.) The standard EN 15804 serves as the core PCR
Independent verification of the declaration and data according to ISO
14025:2011
internally X externally
Florian Pronold Mrs Kim Allbury,
(Managing Director Institut Bauen und Umwelt e.V.) (Independent verifier)
1 Environmental Product Declaration - Grundfos Holding A/S - MAGNA3 65-80/100/120 (Stainless Steel)
Product
Product description/Product definition Ecodesign Directive (2009/125/EC)
The Grundfos MAGNA3 circulator pumps are designed for
circulating liquids in heating systems, air conditioning and Commission Regulation (EC) No: 641/2009 and
cooling systems and domestic hot water systems. However, the
pump range can also be used in ground source heat pump Commission Regulation (EU) 622/2012
systems and solar heating systems.
Standards used:
The MAGNA3 pump is a centrifugal pump powered by an EN 16297-1:2012, EN 16297-2:2012, EN 16297-3:2012.
electrical motor. It has a high-performance neodymium magnet
rotor which increases motor efficiency and an insulation shell to The CE-marking takes into account the proof of conformity with
reduce heat loss from the cast iron pump housing with threaded the respective harmonized norms based on the legal provisions
connections. above.
The declaration covers three types of the MAGNA3 pump. They MAGNA3 pumps are not harmonized in accordance with the
are grouped as shown below. The group reference in the CPR.
technical data and scenarios refers also to these.
Application
GROUP 1 - MAGNA3 65-80 For the application and use the respective national provisions
apply.
GROUP 2 - MAGNA3 65-100 GROUP 3 - MAGNA3 65-120
The pump is designed for circulating liquids in the
These are all the same physical products and 100 % identical
in terms of design, dimensions and materials as well as supply following systems:
chain and manufacturing processes, i.e., all cradle to gate
processes (A1-A3). · heating systems
The products are also identical in terms of packaging, · domestic hot-water systems
distribution, reference service life and end-of-life treatment.
· air-conditioning and cooling systems
The only thing that differentiates the products from each other
is the software which controls how the pump operates in the · ground-source heat-pump systems
system in which it is installed, making them fit for different
applications. Hence, all life cycle modules are identical, except · solar-heating systems
use stage module B6, which will change, as the applied
scenarios for electricity consumption changes. For the placing The pump is suitable for thin, clean, non-aggressive and non-
on the market in the European Union/European Free Trade explosive liquids, not containing solid particles or fibres that
Association (EU/EFTA) (with the exception of Switzerland) the may attack the pump mechanically or chemically. In heating
following legal provisions as well as the corresponding systems, the water must meet the requirements of accepted
harmonised norms based on these provisions apply: standards on water quality in heating systems. The pumps are
Machinery Directive (2006/42/EC) also suitable for domestic hot-water systems
Standard used: EN 809:1998 + A1:2009. Technical Data
The performance data of the product according to the
Radio Equipment Directive (2014/53/EU) harmonized norms, based on the harmonization provisions
above apply.
Standards used:
EN 60335-1:2012/AC:2014 + A11:2014, EN 60335-2-51:2003 + The relevant technical specifications according to the PCR Part
A1:2008 + A2:2012, EN 62233:2008. B are given in the table below.
EN 55014-1:2006 + A1:2009 + A2:2011, EN 55014-1:2017, EN Characteristics that are the same for all product groups are only
61000-6-2:2005, EN 61000-3-2:2014, EN 61000-3-3:2013, given once. Others are given individually for all three groups.
ETSI EN 301 489-1 V2.2.0, ETSI EN 301 489-17 V3.2.0. ETSI Constructional data
EN 300 328 V2.1.1
Electromagnetic Compatibility (EMC) Directive
(2014/30/EU)
Standards used: EN 55014-1:2017, EN 55014-2:2015,
EN 61000-3-2:2014/2019, EN 61000-6-2:2008/2019,
EN 61000-3-3:2013 A1:2019
RoHS Directive 2011/65/EU and 2015/863//EU
Standard: EN 50581:2012.
2 Environmental Product Declaration - Grundfos Holding A/S - MAGNA3 65-80/100/120 (Stainless Steel)
Name ValueUnit REACH
Frequency 50 Hz
This product/article/at least one partial article contains
Voltage 230 V
substances listed in the ECHA candidate list (date:
Energy Efficiency Index Gr.1 0,18
Energy Efficiency Index Gr.2 0,17 10.06.2022) exceeding 0.1 percentage by mass: no
Energy Efficiency Index Gr.3 0,17
Flow range Gr. 1 (max) 37,5 m3/h The Wahlstedt production has been assessed and certified as
meeting the requirements in ISO 14001, ISO 50001, ISO 45001
Flow range Gr. 2 (max) 40,0 m3/h
and ISO 9001.
Flow range Gr. 3 (max) 42,50m3/h
Reference service life
Head max. Gr.1 8 m
No use stage scenario which refers to the lifetime of the product
Head max. Gr.2 10 m
is declared. However, to facilitate building calculations, an
Head max. Gr.3 12 m
estimated RSL of 10 years can be used.
Power input Gr. 1 Average (from load profile This is an EU consensus-based estimation, referenced on page
0,197 kW
describing use) 37 in Appendix 7: Lot 11 – Circulators in Buildings, prepared by
Power input Gr. 2 Average (from load profile AEA Energy & Environment for the European Commission in
0,249 kW
describing use) the context of the Eco Design Directive:
Power input Gr. 3 Average (from load profile
describing use) 0,320 kW There is no definitive information on the average circulator life
available, there is consensus within the industry that it is at
Nominal capacity Gr.1 0,461 kW
least 12 years. However, this is complicated by many factors,
Nominal capacity Gr. 2 0,599 kW
including many being scrapped prematurely when e.g. the
Nominal capacity Gr.3 0,75 kW boiler they are connected to is replaced.
Performance data of the product according to the harmonised
standards, based on provisions for harmonisation. From the estimated stock (140Mpa) and annual sales (14Mpa),
the average lifetime of the circulator is taken as 10 years for the
Base materials/Ancillary materials purposes of this study.
Name Value Unit
The RSL of the declared product is not directly influencing the
Aluminium 13 %
results in this study, as no declared use stage scenario is
Ceramics 0,28 %
dependent on the RSL; The use stage sub-module B6 is
Copper 2,75 % declared per year as required by the PCR Part B.
Electronics 0,21 %
Magnet Nd 1,01 %
Paper 0,46 %
PCB 3,46 %
Plastics 0,31 %
Plastics, foam 1,14 %
Plastics GF 4,78 %
Rubber 0,16 %
Stainless steel 58,26 %
Steel 7,22 %
Cardboard 8 %
Plastic film 0,1 %
TOTAL 100 %
LCA: Calculation rules
Declared Unit The product stage (A1-A3) comprises raw material extraction
The declared and processing, transport processes as well as the
unit is 1 piece (pcs.) of MAGNA3 (Stainless Steel) pump. manufacturing process. The final production and assembly of
Declared unit the MAGNA3 pump takes place at a Grundfos manufacturing
site in Germany. However, the full supply-chain leading to the
Name Value Unit
finished product at the gate is rather complex and includes a
Declared unit 1 pce.
large amount of raw materials, components and semi-finished
Mass reference 24.85 kg/pce parts which comes from both external suppliers as well as other
Conversion factor [Mass/Declared Unit] 24.85 Grundfos production facilities.
System boundary The product stage is included in the study, and according to EN
15804 the system boundary with nature is set to include those
This EPD is Cradle-To-Grave. The system boundaries
processes that provide the material and energy inputs into the
system and the following manufacturing, transport up to the
of the EPD follow the modular approach in EN 15804. By
factory gate as well as the processing any waste arising from
decision no. 20170712-n of the SVR, the modules B3, B4 and
those processes.
B5 are by default declared as "MNR" (module not relevant).
3 Environmental Product Declaration - Grundfos Holding A/S - MAGNA3 65-80/100/120 (Stainless Steel)
Wastes and losses are included in the modules where they · Transport of packaging waste to treatment site;
occur according to the polluter pays principle and the modular
approach of EN 15804. · Waste treatment of packaging.
The product includes: The packaging material does not reach the end of waste state
but is incinerated as waste.
· A1 Extraction and processing of raw materials; According to European statistics, the average R1 value of
incineration plants is > 0.6. Therefore, it is assumed that
· A1 Reuse of products or materials from a previous product packaging material is treated thermally in an incineration plant
system; with R1 > 0.6. The loads from the combustion process of
packaging are declared in module A5 and the resulting energy
· A1 Processing of secondary materials; benefits in module
· A1 Generation of electricity, steam and heat from primary D, as required by the PCR Part A, 5.5.2.
energy resources, also including their extraction, refining and
transport; Use stage (B1-B7):
· A1 Energy recovery and other recovery processes from The use stage, related to the building fabric includes:
secondary fuels;
· B1, use or application of the installed product;
· A2 Transportation up to the factory gate and internal transport;
· B2, maintenance.
· A3 Production of ancillary materials or pre products;
The use stage related to the operation of the building
· A3 Manufacturing of products and coproducts;
includes:
· A3 Manufacturing of packaging;
· B6, operational energy use;
· A1-A3 processing up to the end-of-waste state or disposal of
final residues. · B7, operational water use.
For secondary material inputs, the system boundary to the In this study, all use stage modules are assessed, though B1,
previous system (providing the secondary material) is set where B2 and B7 are assessed to be zero. By decision no. 20170712-
outputs reach the end-of-waste state. The recycling of n of the SVR, the modules B3, B4 and B5 are by default
secondary material into new raw materials is included in the declared as "MNR" (module not relevant).
system boundary of this study. Waste materials from production The modules include the provision and transport of all
processes that are recycled without any modification of the materials, products and related energy and water use, as well
material's inherent characteristics are modelled as closed-loop as waste processing up to the end-of-waste state or disposal of
within A1-A3. This is done up to the input mass flow that was final residues during the use stage. They also include all
used during production. impacts and aspects related to the losses during the use stage
(i.e. production, transport, and waste processing and disposal
Waste for incineration arising in the product stage is accounted of the lost products and materials).
for in the module where the waste is produced. The
environmental loads from the incineration process are declared Generally, the geographical coverage of the datasets used
in the module where it occurs and the electricity and heat which matches the actual processes taking place. Meaning, that when
is produced from the incineration are considered as closed-loop modelling taking place in Grundfos Bjerringbro, the Danish
within A1-A3, as described in PCR Part A, 5.5.1. The input of electricity grid mix is used in the model and thermal energy
biogenic carbon from the production of packaging material is from natural gas. These are generally of very high quality with
inventoried in A3. As required by PCR Part A, the very good technological, temporal and geographical
corresponding end-of-life module of the packaging material, A5, representativeness.
is also declared and the emissions of biogenic carbon are
inventoried. Contributions to operational energy use during the use stage
(B6) come from the electricity consumption of the product. The
The construction process stage (A4-A5) includes: annual electricity consumption is calculated by multiplying the
average power input, which is based on a defined load profile,
A4: with the annual running hours. For use stage (B6) European
Average electricity grid mix has been used. These values are
· Transportation from factory gate to the distribution center: declared in the scenarios section.
· Consumption of electricity, thermal energy and water at the The End-of-Life stage (C1-C4) includes all activities from
distribution center; when the product reaches the end of its service life and no
longer provides any functionality and until all materials and
· Transportation from distribution center to construction site; components are processed for reuse/recycling or disposed of.
· Wastage during distribution. According to EN 15804 and the PCR Part A, the end-of-life
stage includes:
A5:
· C1 deconstruction of the product from the
· Installation process;
4 Environmental Product Declaration - Grundfos Holding A/S - MAGNA3 65-80/100/120 (Stainless Steel)
· building, including initial on-site sorting of the Beyond system boundary (D): According to EN 15804
module D includes the reuse, recovery and/or recycling
· materials; potentials, expressed as net impacts and benefits. Any
declared benefits and loads from net
· C2 transportation of the discarded product to a recycling site
and transportation of waste to final disposal; flows leaving the product system that have not been allocated
as co-products and that have passed the end-of-waste state
· C3 waste processing, collection of waste fractions from the are included in module D.
deconstruction and waste processing of material flows intended
for reuse, recycling and energy recovery; Contributions to module D comes from waste incineration
processes in A5 and C3 as well as material recycling in C3. The
· C4 waste disposal including physical pretreatment and specific fractions and net flows are shown in the scenarios
management of the disposal site. section.
At the end of life, the MAGNA3 pump is manually disassembled Comparability
from the piping system in which it has been installed. The
definition of the applied end-of-life scenario in this EPD follows Basically, a comparison or an evaluation of EPD data is only
the requirements in the possible if all the data sets to be compared were created
according to EN 15804 and the building context, respectively
PCR Part A, 6.2 regarding complex products, with a the product-specific characteristics of performance, are taken
combination of recycling, thermal waste treatment and into account.
landfilling. 100 % of the material is considered in the end of life
scenario as required by the PCR. An overall collection rate of Geographic Representativeness
90 % has been assumed. Land or region, in which the declared product system is
manufactured, used or handled at the end of the product´s
Materials from which energy is recovered in an incineration lifespan: Germany
process with an R1-value above 0.60 are in this study included
with the environmental burdens from the incineration process
Comparability
inventoried in C3, the recovered energy is declared as exported
Basically, a comparison or an evaluation of EPD data is only
energy in C3 and the energy benefits are declared in D. This
possible if all the data sets to be compared were created
procedure is according to the PCR Part A, 5.5.6. C3 includes
according to EN 15804 and the building context, respectively
the mechanical separation of the product followed by a series
the product-specific characteristics of performance, are taken
of sorting steps. Metal fractions are recycled and plastics,
into account. Software and databases used: LCA for Experts
cardboard and electronics are assumed incinerated with energy
10.7.1.28
recovery. The residual fractions are landfilled and declared in
Schema 8007
C4.
Sphera and Ecoinvent databases
The specific amounts are shown in the scenarios section.
LCA: Scenarios and additional technical information
Name Value Unit
Characteristic product properties of biogenic carbon
Litres of fuel 0,0332 l/100km
The biogenic carbon content quantifies the amount of biogenic
Transport distance 2003 km
carbon in a construction product leaving the factory gate, and it
will be separately declared for the product and for any Capacity utilisation (including empty runs) 85 %
accompanying packaging, as required from the PCR Part A. Gross density of products transported 460 kg/m3
The Carbon content of Cardboard and Paper is assumed to
Wastage during distribution 0,02 %
0.46 kg in 1 kg of material. This means that 46% biogenic
carbon content is assumed Overall, there is an amount of Installation into the building (A5)
weight-% Carbon in the product leaving the factory gate and
Name ValueUnit
has to be considered
Packaging waste for incineration (LDPE film) 0,02 kg
Packaging waste for incineration
Information on describing the biogenic Carbon Content at 1,955 kg
(Paper/Cardboard)
factory gate
An estimated RSL of 10 years can be used to facilitate building
Name ValueUnit
calculations. This is an EU consensus-based estimation,
Biogenic carbon content in accompanying kg
0.9 referenced in Appendix 7: Lot 11 – Circulators in Buildings,
packaging C
prepared by AEA Energy & Environment for the European
Note: 1 kg of biogenic carbon is equivalent to 44/12 kg of CO2 Commission in the context of the Eco Design Directive.
Reference service life
Name Value Unit
Transport from the gate to the site (A4)
Life Span according to the manufacturer 10 a
Operational energy use (B6)
5 Environmental Product Declaration - Grundfos Holding A/S - MAGNA3 65-80/100/120 (Stainless Steel)
Name Value Unit Reuse, recovery and/or recycling potentials (D), relevant
Electricity consumption Group 1 985 kWh/a scenario information
Electricity consumption Group 2 1245 kWh/a Name Value Unit
Electricity consumption Group 3 1600 kWh/a A5, incineration w/energy recov. thermal energy 8,89 MJ
Average power input, Group 1 0,197 kW A5, incineration w/energy recov. electric energy 4,91 MJ
Average power input, Group 2 0,249 kW C3, steel for recycling (net amounts) -0,469 kg
Average power input, Group 3 0,32 kW C3, stainless steel for recycling (net amounts) 3,93 kg
Running hours (all groups) 5.000 h/a C3, aluminium for recycling (net amounts) -0,436 kg
C3, copper for recycling (net amounts) 0,258 kg
End of life (C1-C4)
C3, incineration w/energy recov. thermal energy 13,4 MJ
Name Value Unit
C3, incineration w/energy recov. electric energy 7,45 MJ
Collected as mixed construction waste 22,871 kg
Transportation distance (C2) 500 km
Aluminium for recycling 2,74 kg
Steel for recycling 1,58 kg
Copper for recycling 0,60 kg
Stainless steel for recycling 12,76 kg
Plastics for incineration w/energy 1,40 kg
Electronics for incineration w/energy 0,80 kg
Landfilling 2,81 kg
6 Environmental Product Declaration - Grundfos Holding A/S - MAGNA3 65-80/100/120 (Stainless Steel)
LCA: Results
Characterization model: EN 15804 - 2012+A2 - 2019, PEF. By Decision no. 20170712-n of the IBU SVR, the modules B3, B4, B5 are
marked as MNR (module not relevant) as default. The LCA results in module B6 are given on a period of one year, according to PCR
Part B. To obtain the results from module B6 over the entire life cycle, the LCA results of module B6 must be multiplied by the
estimated RSL of 10 years. The indicator results for module B6 are declared for Group 1. B6 indicator results for other groups can be
derived by multiplying the B6 indicator results with the following factors:
GROUP 1 - MAGNA3 65-80: 1,00
GROUP 2 - MAGNA3 65-100: 1,265
GROUP 3 - MAGNA3 65-120: 1,626
DESCRIPTION OF THE SYSTEM BOUNDARY (X = INCLUDED IN LCA; MND = MODULE OR INDICATOR NOT DECLARED; MNR
= MODULE NOT RELEVANT)
Benefits and
Construction loads beyond
Product stage Use stage End of life stage
process stage the system
boundaries
la ire ta m w a Ry lp p u s tro p s n a rT g n iru tc a fu n a M e h t m o rf tro p s n a rTe tis e h t o t e ta g y lb m e s s A e s U e c n a n e tn ia M ria p e R tn e m e c a lp e R tn e m h s ib ru fe R y g re n e la n o ita re p Oe s u re ta w la n o ita re p Oe s u n o itc u rts n o c -e Dn o itilo m e d tro p s n a rT g n is s e c o rp e ts a W la s o p s iD -e s u e R-y re v o c e R-g n ilc y c e Rla itn e to p
A1 A2 A3 A4 A5 B1 B2 B3 B4 B5 B6 B7 C1 C2 C3 C4 D
X X X X X X X MNR MNR MNR X X X X X X X
RESULTS OF THE LCA - ENVIRONMENTAL IMPACT according to EN 15804+A2: 1PCS of MAGNA3 65-80/100/120
Parameter Unit A1 A2 A3 A4 A5 B1 B2 B6 B7 C1 C2 C3 C4 D
GWP-total kg CO 2 eq 1.19E+02 6.12E+00 6.92E-01 1.9E+00 3.17E+00 0 0 3.21E+02 0 0 7.85E-01 6.32E+00 1.46E-01 -1.21E+01
GWP-fossil kg CO 2 eq 1.18E+02 6.12E+00 3.91E+00 1.91E+00 4.68E-01 0 0 3.18E+02 0 0 7.89E-01 6.3E+00 1.48E-01 -1.21E+01
GWP- -3.25E
biogenic kg CO 2 eq -1.82E-02 -9.84E-03 +00 -2.81E-02 2.7E+00 0 0 2.76E+00 0 0 -1.17E-02 1.59E-02 -1.83E-03 -3.14E-02
GWP-luluc kg CO 2 eq 7.48E-02 9.29E-03 3.04E-02 1.73E-02 9.55E-05 0 0 3.45E-02 0 0 7.33E-03 2.34E-04 1.34E-04 -3.16E-03
kg CFC11
ODP 4.74E-08 4.8E-13 4.06E-09 1.07E-11 4.18E-13 0 0 5.86E-09 0 0 1.03E-13 3.45E-11 2.47E-13 -2.44E-11
eq
AP mol H+ eq 8.61E-01 1.82E-01 1.94E-02 1.14E-02 8.6E-04 0 0 6.79E-01 0 0 4.75E-03 4.74E-03 4.57E-04 -1.12E-01
EP-
kg P eq 1.52E-03 4.79E-06 6.86E-05 7.18E-06 1.56E-07 0 0 1.19E-03 0 0 2.89E-06 9.76E-06 1.7E-05 -1.55E-05
freshwater
EP-marine kg N eq 9.35E-02 4.34E-02 4.06E-03 5.5E-03 3.15E-04 0 0 1.62E-01 0 0 2.31E-03 1.23E-03 1.09E-04 -1.31E-02
EP-terrestrial mol N eq 1.01E+00 4.76E-01 4.07E-02 6.1E-02 3.95E-03 0 0 1.7E+00 0 0 2.57E-02 1.38E-02 1.2E-03 -1.41E-01
kg
POCP NMVOC 2.97E-01 1.23E-01 1.14E-02 1.05E-02 8.18E-04 0 0 4.33E-01 0 0 4.39E-03 3.29E-03 3.44E-04 -4.21E-02
eq
ADPE kg Sb eq 9.16E-03 1.13E-07 6.05E-05 1.97E-06 4.3E-09 0 0 4.91E-05 0 0 5.24E-08 2.88E-07 3.98E-09 -1.32E-03
ADPF MJ 1.66E+03 7.61E+01 5.8E+01 2.62E+01 1.16E+00 0 0 6.69E+03 0 0 1.08E+01 4.01E+01 2.21E+00 -1.4E+02
m3 world
WDP eq 3.94E+01 2.05E-02 3.94E-02 3.19E-02 3.81E-01 0 0 7.08E+01 0 0 9.56E-03 8.66E-01 -2.06E-03 -8E-01
deprived
GWP = Global warming potential; ODP = Depletion potential of the stratospheric ozone layer; AP = Acidification potential of land and water; EP =
Eutrophication potential; POCP = Formation potential of tropospheric ozone photochemical oxidants; ADPE = Abiotic depletion potential for non-fossil
resources; ADPF = Abiotic depletion potential for fossil resources; WDP = Water (user) deprivation potential)
RESULTS OF THE LCA - INDICATORS TO DESCRIBE RESOURCE USE according to EN 15804+A2: 1PCS of MAGNA3 65-
80/100/120
Parameter Unit A1 A2 A3 A4 A5 B1 B2 B6 B7 C1 C2 C3 C4 D
PERE MJ 4.3E+02 1.26E+00 5.58E+01 2.03E+00 2.61E-01 0 0 4E+03 0 0 7.84E-01 2.35E+01 1.99E-01 3.04E+00
PERM MJ 0 0 0 0 0 0 0 0 0 0 0 0 0 0
PERT MJ 1.26E+00 5.58E+01 2.03E+00 2.61E-01 0 0 0 4E+03 0 0 7.84E-01 2.35E+01 1.99E-01 3.04E+00
PENRE MJ 1.66E+03 7.63E+01 5.8E+01 2.62E+01 1.16E+00 0 0 6.69E+03 0 0 1.08E+01 4.02E+01 2.22E+00 -1.4E+02
PENRM MJ 0 0 0 0 0 0 0 0 0 0 0 0 0 0
PENRT MJ 1.66E+03 7.63E+01 5.8E+01 2.62E+01 1.16E+00 0 0 6.69E+03 0 0 1.08E+01 4.02E+01 2.22E+00 -1.4E+02
SM kg 1.46E+01 0 2.31E-01 2.97E-03 0 0 0 0 0 0 0 0 0 0
RSF MJ 1.46E-23 0 0 2.91E-27 0 0 0 0 0 0 0 0 0 0
NRSF MJ 1.71E-22 0 0 3.42E-26 0 0 0 0 0 0 0 0 0 0
FW m3 1.17E+00 1.44E-03 2.32E-02 2.32E-03 8.98E-03 0 0 3.23E+00 0 0 8.59E-04 2.94E-02 2.31E-05 2.05E-02
PERE = Use of renewable primary energy excluding renewable primary energy resources used as raw materials; PERM = Use of renewable primary
energy resources used as raw materials; PERT = Total use of renewable primary energy resources; PENRE = Use of non-renewable primary energy
excluding non-renewable primary energy resources used as raw materials; PENRM = Use of non-renewable primary energy resources used as raw
materials; PENRT = Total use of non-renewable primary energy resources; SM = Use of secondary material; RSF = Use of renewable secondary fuels;
7 Environmental Product Declaration - Grundfos Holding A/S - MAGNA3 65-80/100/120 (Stainless Steel)
NRSF = Use of non-renewable secondary fuels; FW = Use of net fresh water
RESULTS OF THE LCA – WASTE CATEGORIES AND OUTPUT FLOWS according to EN 15804+A2:
1PCS of MAGNA3 65-80/100/120
Parameter Unit A1 A2 A3 A4 A5 B1 B2 B6 B7 C1 C2 C3 C4 D
HWD kg 7.01E-06 2.4E-10 1.21E-04 2.57E-08 2.94E-11 0 0 7.86E-07 0 0 3.35E-11 4.56E-09 1.85E-10 -2.44E-03
NHWD kg 9.4E+00 7.8E-03 3.75E-01 6.09E-03 1.23E-01 0 0 4.9E+00 0 0 1.65E-03 6.6E-01 2.56E+00 2.1E+00
RWD kg 5.61E-02 9.91E-05 1.78E-03 6.49E-05 5.29E-05 0 0 1.06E+00 0 0 2.02E-05 6.23E-03 2.6E-05 -2.52E-03
CRU kg ND ND ND ND ND ND ND ND ND ND ND ND ND ND
MFR kg 0 0 0 0 0 0 0 0 0 0 0 1.77E+01 0 0
MER kg ND ND ND ND ND ND ND ND ND ND ND ND ND ND
EEE MJ 0 0 0 0 4.91E+00 0 0 0 0 0 0 7.45E+00 0 0
EET MJ 0 0 0 0 8.89E+00 0 0 0 0 0 0 1.34E+01 0 0
HWD = Hazardous waste disposed; NHWD = Non-hazardous waste disposed; RWD = Radioactive waste disposed; CRU = Components for re-use;
MFR = Materials for recycling; MER = Materials for energy recovery; EEE = Exported electrical energy; EET = Exported thermal energy
RESULTS OF THE LCA – additional impact categories according to EN 15804+A2-optional:
1PCS of MAGNA3 65-80/100/120
Parameter Unit A1 A2 A3 A4 A5 B1 B2 B6 B7 C1 C2 C3 C4 D
Disease
PM 1.08E-05 3.15E-06 2.88E-07 7.41E-08 5.08E-09 0 0 5.71E-06 0 0 3.01E-08 3.01E-08 4.64E-09 -2.74E-06
incidence
kBq U235
IR 7.53E+00 1.43E-02 2.85E-01 9.58E-03 8.25E-03 0 0 1.77E+02 0 0 3.02E-03 3.02E-03 3.85E-03 -2.13E-01
eq
ETP-fw CTUe 8.38E+02 5.39E+01 1.98E+01 1.84E+01 5.58E-01 0 0 1.86E+03 0 0 7.72E+00 7.72E+00 1.39E+00 -1.82E+01
HTP-c CTUh 2.38E-05 1E-09 6.46E-07 5.27E-09 3.05E-11 0 0 9.84E-08 0 0 1.57E-10 1.57E-10 8.93E-11 -5.37E-07
HTP-nc CTUh 1.79E-06 3.45E-08 4.24E-08 1.69E-08 1.14E-09 0 0 1.57E-06 0 0 6.97E-09 6.97E-09 7.63E-09 -7.24E-08
SQP SQP 3.87E+02 5.86E+00 1.06E+02 1.08E+01 3.41E-01 0 0 2.62E+03 0 0 4.5E+00 4.5E+00 1.98E-01 -1.85E+01
PM = Potential incidence of disease due to PM emissions; IR = Potential Human exposure efficiency relative to U235; ETP-fw = Potential comparative
Toxic Unit for ecosystems; HTP-c = Potential comparative Toxic Unit for humans (cancerogenic); HTP-nc = Potential comparative Toxic Unit for humans
(not cancerogenic); SQP = Potential soil quality index
Disclaimer 1 – for the indicator 'Potential Human exposure efficiency relative to U235'.
This impact category deals mainly with the eventual impact of low-dose ionizing radiation on human health of the nuclear fuel cycle. It
does not consider effects due to possible nuclear accidents, occupational exposure or radioactive waste disposal in underground
facilities. Potential ionizing radiation from the soil, radon and from some construction materials is also not measured by this indicator.
Disclaimer 2 – for the indicators 'abiotic depletion potential for non-fossil resources', 'abiotic depletion potential for fossil resources',
'water (user) deprivation potential, deprivation-weighted water consumption', 'potential comparative toxic unit for ecosystems', 'potential
comparative toxic unit for humans – cancerogenic', 'Potential comparative toxic unit for humans - not cancerogenic', 'potential soil
quality index'. The results of this environmental impact indicator shall be used with care as the uncertainties on these results are high
as there is limited experience with the indicator.
Disclaimer 3: JRC Technical Reports, Version 2, 2018 Page 6, for the indicator "EP-freshwater". This indicator has been calculated as
'kg P eq' as required in the characterization model EUTREND model, Struijs et al., 2009b, as implemented in ReCiPe; This EPD was
created using a software tool.
References
Standards PARLIAMENT AND OF THE COUNCIL of 26 February
Machinery Directive 2014 on the harmonistion of the laws of the Member
DIRECTIVE 2006/42/EC OF THE EUROPEAN States relating to electromagnetic compatibility
PARLIAMENT AND OF THE COUNCIL of 17 May Ecodesign Directive
2006 on machinery DIRECTIVE 2009/125/EC OF THE EUROPEAN
Radio Equipment Directive PARLIAMENT AND OF THE COUNCIL of 21 October
DIRECTIVE 2014/53/EU OF THE EUROPEAN PARLIAMENT 2009 establishing a framework for the setting of
AND OF THE COUNCIL of 16 April 2014 on the harmonisation
of the laws of the Member States relating to the making ecodesign requirements for energy-related products
available on the market of
EC 641/2009
radio equipment
COMMISSION REGULATION (EC) No 641/2009 of 22 July
Electromagnetic Compatibility (EMC) Directive 2009 implementing Directive 2005/32/EC of the European
Parliament and of the Council with regard to ecodesign
DIRECTIVE 2014/30/EU OF THE EUROPEAN requirements for glandless standalone circulators and
glandless circulators integrated in
8 Environmental Product Declaration - Grundfos Holding A/S - MAGNA3 65-80/100/120 (Stainless Steel)
EN 50581:2012
products
EN 50581:2012, Technical documentation for the
EC 622/2012
assessment of electrical and electronic products with
COMMISSION REGULATION (EU) No 622/2012 of 11 July
2012 amending Regulation (EC) No 641/2009 with regard to respect to the restriction of hazardous substances
ecodesign requirements for glandless standalone circulators
and glandless circulators integrated in products EN 60335-1
DIRECTIVE 2011/65/EU EN 60335-1:2012/A11:2014/A13:2017, Household
DIRECTIVE 2011/65/EU OF THE EUROPEAN and similar electrical appliances – Safety – Part 1:General
requirements
PARLIAMENT AND OF THE COUNCIL of 8 June 2011
EN 60335-2-51
on the restriction of the use of certain hazardous
EN 60335-2-51:2003-03 + A1:2008 + A2:2012, Household and
substances in electrical and electronic equipment similar electrical appliances – Safety –Part 2-51: Particular
requirements for stationary circulation pumps for heating and
DIRECTIVE 2015/863/EU service water installations
DIRECTIVE 2015/863/EU of 31 March 2015 amending EN 61000-3-2
Annex II to Directive 2011/65/EU of the European EN 61000-3-2:2014/2019, Electromagnetic compatibility (EMC)
– Part 3-2: Limits – Limits for harmonic current emissions
Parliament and of the Council as regards the list of (equipment input current =16 A per phase)
restricted substances EN 61000-3-3
ETSI EN 301 489-1 EN 61000-3-3:2013-08/ A1:2019, Electromagnetic compatibility
(EMC) – Part 3-3:
ETSI EN 301 489-1 V2.2.0, Electromagnetic Compatibility Limits – Limitation of voltage changes, voltage fluctuations and
(EMC) standard for radio equipment and services; Part 1: flicker in public low voltage supply systems, for equipment with
Common technical requirements
rated current <= 16 A per phase and not subject to conditional
ETSI EN 301 489-17 connection
ETSI EN 301 489-17 V3.2.0, Electromagnetic Compatibility EN 61000-6-2
(EMC) standard for radio equipment and services; Part 17:
Specific conditions for Broadband Data Transmission Systems EN 61000-6-2:2008/2019, Electromagnetic compatibility (EMC)
– Part 6-2: Generic standards –Immunity for industrial
ETSI EN 300 328 V2.1.1 environments
ETSI EN 300 328 V2.1.1, Wideband transmission systems; EN 16297-1
Data transmission equipment operating in the 2,4 GHz ISM
band and using wide band modulation techniques EN 16297-1:2012-10, Pumps – Rotodynamic pumps –
Glandless circulators – Part 1:
EN 809 General requirements and procedures for testing and
calculation of energy efficiency index (EEI)
EN 809:1998-10 + A1:2009, Pumps and pump units for
EN 16297-2
liquids - Common safety requirements
EN 16297-2:2012-10, Pumps – Rotodynamic pumps –
EN 55014-1 Glandless circulators – Part 2: Calculation of energy efficiency
index (EEI) for standalone circulators
EN 55014-1:2017, Electromagnetic compatibility –
Requirements for household appliances, electric tools and EN 16297-3
similar apparatus – Part 1: Emission
EN 16297-3:2012, Pumps – Rotodynamic pumps –Glandless
EN 55014-2 circulators – Part 3: Energy efficiency index (EEI) for circulators
integrated in products
EN 55014-2:2015, Electromagnetic compatibility –
ISO 14001
Requirements for household appliances, electric tools
EN ISO 14001:2015-09, Environmental management systems -
and similar apparatus – Part 2: Immunity – Product Requirements with guidance for use
family standard (CISPR 14-2:2015) ISO 14025
9 Environmental Product Declaration - Grundfos Holding A/S - MAGNA3 65-80/100/120 (Stainless Steel)
DIN EN /ISO 14025:2011-10, Environmental labels and
declarations — Type III environmental declarations — Impact assessment characterization factors Institute of
Principles and procedures Environmental Sciences, Leiden University, Netherlands
EN 15804 ECHA candidate list
EN 15804:2012-04+A1 2013, Sustainability of construction Candidate List of substances of very high concern (SVHCs) for
works — Environmental Product Declarations — Core rules for authorisation, European Chemicals Agency (ECHA), Helsinki,
the product category of construction products Finland
PCR Part A EUTREND model
Institut Bauen und Umwelt e.V., Berlin (pub.): Product Category Struijs et al., 2009b
Rules for Building-Related Products and Services, Product
Category Rules for Construction Products from the range of
Environmental Product Declarations of Institut Bauen und AEA Energy & Environment
Umwelt (IBU), Part A: Calculation Rules for the Life Cycle
Assessment and Requirements on the Project Report, Version Circulators in Buildings
1.3.
Ecoinvent
PCR Part B
Ecoinvent v3.9.1
Institut Bauen und Umwelt e.V., Berlin (pub.): Product Category
Rules for Building-Related Products and Services, Product LCA for Experts
Category Rules for Construction Products from the range of
Environmental Product Declarations of Institut Bauen und LCA for Experts 10.7.1.28Schema 8007
Umwelt (IBU), Part B: Requirements on the EPD for Pumps for
liquids and liquids with solids, Version 1.0 (2018) REACH
Regulation (EC) No 1907/2006 of the European Parliament and
Further references of the Council of 18 December 2006 concerning the
Registration, Evaluation, Authorisation and Restriction of
CPR Chemicals (REACH) (Status: 27.06.2018)
REGULATION (EU) No 305/2011 OF THE EUROPEAN SVR
PARLIAMENT AND OF THE COUNCIL of 9 March 2011 laying
down harmonised conditions for the marketing of construction Advisory Board (formerly SVA)
products and repealing Council Directive 89/106/EEC
Decision no.
CML 2001 20170712-n
10 Environmental Product Declaration - Grundfos Holding A/S - MAGNA3 65-80/100/120 (Stainless Steel)
Publisher
Institut Bauen und Umwelt e.V. +49 (0)30 3087748- 0
Hegelplatz 1 info@ibu-epd.com
10117 Berlin www.ibu-epd.com
Germany
Programme holder
Institut Bauen und Umwelt e.V. +49 (0)30 3087748- 0
Hegelplatz 1 info@ibu-epd.com
10117 Berlin www.ibu-epd.com
Germany
Author of the Life Cycle Assessment
Grundfos Holding A/S +45 87501400
Poul Due Jensens Vej 7 LCA_EPD@grundfos.com
8850 Bjerringbro www.grundfos.com
Denmark
Owner of the Declaration
Grundfos Holding A/S +45 87501400
Poul Due Jensens Vej 7 LCA_EPD@grundfos.com
8850 Bjerringbro www.grundfos.com
Denmark
11 Environmental Product Declaration - Grundfos Holding A/S - MAGNA3 65-80/100/120 (Stainless Steel)
