ENVIRONMENTAL PRODUCT DECLARATION
as per ISO 14025 and EN 15804+A2
Owner of the Declaration dormakaba International Holding GmbH
Publisher Institut Bauen und Umwelt e.V. (IBU)
Programme holder Institut Bauen und Umwelt e.V. (IBU)
Declaration number EPD-DOR-20240264-CBA1-EN
Issue date 29.11.2024
Valid to 28.11.2029
Door closer TS Compakt
dormakaba
www.ibu-epd.com | https://epd-online.com
General Information
dormakaba Door closer TS Compakt
Programme holder Owner of the declaration
IBU – Institut Bauen und Umwelt e.V. dormakaba International Holding GmbH
Hegelplatz 1 DORMA Platz 1
10117 Berlin 58256 Ennepetal
Germany Germany
Declaration number Declared product / declared unit
EPD-DOR-20240264-CBA1-EN 1 piece of the product: Door closer TS Compakt consisting of the following
items:
• 1 door closer
• Product packaging
This declaration is based on the product category rules: Scope:
Building Hardware products, 01.08.2021 This Environmental Product Declaration refers to a specific door closer
(PCR checked and approved by the SVR) manufactured by dormakaba. The production site is located in Suzhou
(China).
Issue date The data represents the year 2022.
29.11.2024
The owner of the declaration shall be liable for the underlying information
and evidence; the IBU shall not be liable with respect to manufacturer
information, life cycle assessment data and evidences.
Valid to
28.11.2029 The EPD was created according to the specifications of EN 15804+A2. In
the following, the standard will be simplified as EN 15804.
Verification
The standard EN 15804 serves as the core PCR
Independent verification of the declaration and data according to ISO
14025:2011
internally X externally
Dipl.-Ing. Hans Peters
(Chairman of Institut Bauen und Umwelt e.V.)
Florian Pronold Matthias Klingler,
(Managing Director Institut Bauen und Umwelt e.V.) (Independent verifier)
1 Environmental Product Declaration - dormakaba - Door closer TS Compakt
Product
technicalprovision which can be applied are mentioned above.
Product description/Product definition
With the door closer TS Compakt, dormakaba has developed a Base materials/Ancillary materials
door closer which can be universally used on all common door The major material composition including the packaging of the
types. It is particularly quick and easy to install – and does not product is listed below:
require a mounting backplate. Changes in templating allow Name Value Unit
easy selection of the closing force to suit various door sizes.
Steel 61 %
Aluminium 25 %
For the use and application of the product the respective
national provisions at the place of use apply. For the door Lubricant 7 %
closer TS Compakt the standards which can be applied are the Packaging 5 %
following: Plastics <1 %
• EN 1634-1 Paper <1 %
• UL 10c
The product includes partial articles which contain substances
...
listed in the Candidate List of REACH Regulation
Application 1907/2006/EC (date: 14.06.2023) exceeding 0.1 percentage by
mass: yes
The door closer TS Compakt is the ideal solution for standard
doors. • Lead (Pb): 7439-92-1 (CAS-No.) is included in some of
the alloys used. The concentration of lead in each
Technical Data individual alloy does not exceed 4% (by mass).
The door closer TS Compakt has following technical properties:
The Candidate List can be found on the ECHA website
Name Value Unit address: https:echa.europa.eu/de/home.
Closing force 2/3/4 adjustable
Reference service life
For standard doors 1100 mm
The reference service life of the door closer TS Compakt
Non-handed NA standard
amounts to 10 years, depending on the application and
Hold-open function NA optional frequency of use. For repairs and renewals, suitable spare
Closing speed NA adjustable parts are available. The door closer is tested and certified to
Closing speed range 180-15/15-0 deegres UL10c, meaning they are designed to withstand a minimum of
100,000 cycles.
Performance data of the product with respect to its
characteristics in accordance with the relevant
LCA: Calculation rules
— A4, transport to the building site; — A5, installation into the
Declared Unit building; including provision of all materials, products and
energy, as well as waste processing up to the end-of-waste
The declared unit is 1 piece of the product: Door closer TS state or disposal of final residues during the construction
Compakt including packaging process stage.
Name Value Unit
End-of-life stage– Modules C1-C4 and D
Declared unit 1 piece/product
The end-of-life stage includes: — C1, de-construction,
Mass of declared product without
1.23 kg demolition: — C2, transport to waste processing; — C3, waste
packaging
processing for reuse, recovery and/or recycling; — C4,
Mass of packaging 0,07 kg
disposal; including provision and all transport, provision of all
materials, products and related energy and water use. Module
D (Benefits and loads beyond the system boundary) includes:
System boundary — D, recycling potentials, expressed as net impacts and
The type of EPD is: cradle to gate with options, modules C1– benefits.
C4, and module D (A1–A3 + C + D and additional modules:
A4+ A5) Geographic Representativeness
Land or region, in which the declared product system is
Production - Module A1-A3 manufactured, used or handled at the end of the product´s
The product stage includes: — A1, raw material extraction, lifespan: Global
processing and mechanical treatments, processing of
secondary material input (e.g. recycling processes), — A2,
Comparability
transport to the manufacturer, — A3, manufacturing and
Basically, a comparison or an evaluation of EPD data is only
assembly including provision of all materials, products and
possible if all the data sets to be compared were created
energy, as well as waste processing up to the end-of-waste
according to EN 15804 and the building context, respectively
state.
the product-specific characteristics of performance, are taken
into account. Background database: GaBi, SP40.
Construction stage - Modules A4-A5
The construction process stage includes:
2 Environmental Product Declaration - dormakaba - Door closer TS Compakt
LCA: Scenarios and additional technical information
Installation into the building (A5)
Characteristic product properties of biogenic carbon
Name Value Unit
Name ValueUnit Waste packaging (paper and plastic) 0.07 kg
kg
Biogenic carbon content in product -
C
Reference service life
Biogenic carbon content in accompanying kg
0.03 Name Value Unit
packaging C
Life Span according to the manufacturer 10 a
Note: 1 kg of biogenic carbon is equivalent to 44/12 kg of CO .
2
End of life (C1-C4)
C1: The product dismantling from the building is done manually
Suzhou (China) is considered for A3. without environmental burden.
C2: Transport to waste management is 50 km.
Transport to the building site (A4) Name Value Unit
Name Value Unit Collected separately waste type 1.23 kg
Litres of fuel 0.00276l/100km Recycling 1.23 kg
Capacity utilisation (including empty runs) 55 % Energy recovery 0.0017 kg
Transport distance (ship) 10000 km The product is disassembled in a recycling process. Material
Transport distance via truck (from habor to recycling is then assumed for metals. The plastic components
500 km
dormakaba logistic centre) are assumed to be incinerated with energy recovery. Region for
Transport distance via truck (for scaling) 100 km the End of Life is: Global.
The product is transported via truck and ship. The main
Reuse, recovery and/or recycling potentials (D), relevant
distribution regions are Asia and the EU (Russia). For Asia and
scenario information
Russia, the product is stored in China with the calculated
transport distances. For the rest of Europe, the product is Name Value Unit
stored in the dormakaba logistic center in Germany. In order to Recycling 100 %
allow scaling to a specific point of installation 100 km is
The collection rate is 100 %.
declared as well.
3 Environmental Product Declaration - dormakaba - Door closer TS Compakt
LCA: Results
DESCRIPTION OF THE SYSTEM BOUNDARY (X = INCLUDED IN LCA; MND = MODULE OR INDICATOR NOT DECLARED; MNR
= MODULE NOT RELEVANT)
Benefits and
Construction loads beyond
Product stage Use stage End of life stage
process stage the system
boundaries
la ire ta m w a Ry lp p u s tro p s n a rT g n iru tc a fu n a M e h t m o rf tro p s n a rTe tis e h t o t e ta g y lb m e s s A e s U e c n a n e tn ia M ria p e R tn e m e c a lp e R tn e m h s ib ru fe R y g re n e la n o ita re p Oe s u re ta w la n o ita re p Oe s u n o itc u rts n o c -e Dn o itilo m e d tro p s n a rT g n is s e c o rp e ts a W la s o p s iD -e s u e R-y re v o c e R-g n ilc y c e Rla itn e to p
A1 A2 A3 A4 A5 B1 B2 B3 B4 B5 B6 B7 C1 C2 C3 C4 D
X X X X X MND MND MNR MNR MNR MND MND X X X X X
RESULTS OF THE LCA - ENVIRONMENTAL IMPACT according to EN 15804+A2: 1 piece TS Compakt
Parameter Unit A1-A3 A4 A5 C1 C2 C3 C4 D
GWP-total kg CO 2 eq 1.15E+01 9.93E-02 9.81E-02 0 5.38E-03 2.22E-01 0 -2.46E+00
GWP-fossil kg CO 2 eq 1.17E+01 9.67E-02 2.46E-03 0 5.14E-03 2.11E-01 0 -2.45E+00
GWP-biogenic kg CO 2 eq -1.18E-01 2.57E-03 9.57E-02 0 2.38E-04 1.08E-02 0 -7.48E-03
GWP-luluc kg CO 2 eq 4.68E-03 2.17E-06 1.61E-06 0 1.22E-07 1.2E-05 0 -4.13E-04
ODP kg CFC11 eq 2.3E-12 9.74E-18 1.77E-17 0 5.43E-19 1.08E-16 0 -1.71E-11
AP mol H+ eq 5.42E-02 1.62E-03 2.75E-05 0 5.15E-06 3.91E-05 0 -8.81E-03
EP-freshwater kg P eq 6.91E-06 2.12E-08 3.46E-09 0 1.1E-09 1.71E-08 0 -1.44E-06
EP-marine kg N eq 9.06E-03 4.3E-04 9.92E-06 0 1.64E-06 8.97E-06 0 -1.19E-03
EP-terrestrial mol N eq 9.84E-02 4.72E-03 1.24E-04 0 1.82E-05 1.78E-04 0 -1.29E-02
kg NMVOC
POCP 2.79E-02 1.2E-03 2.63E-05 0 4.63E-06 2.48E-05 0 -3.84E-03
eq
ADPE kg Sb eq 1.29E-04 2.72E-09 2.79E-10 0 1.54E-10 1.48E-09 0 -2.66E-05
ADPF MJ 1.19E+02 1.28E+00 3.1E-02 0 7.29E-02 1E-01 0 -3.43E+01
m3 world eq
WDP 2.19E+00 1.83E-04 1.22E-02 0 1.01E-05 2.27E-02 0 -1.27E-01
deprived
GWP = Global warming potential; ODP = Depletion potential of the stratospheric ozone layer; AP = Acidification potential of land and water; EP =
Eutrophication potential; POCP = Formation potential of tropospheric ozone photochemical oxidants; ADPE = Abiotic depletion potential for non-fossil
resources; ADPF = Abiotic depletion potential for fossil resources; WDP = Water (user) deprivation potential)
RESULTS OF THE LCA - INDICATORS TO DESCRIBE RESOURCE USE according to EN 15804+A2: 1 piece TS Compakt
Parameter Unit A1-A3 A4 A5 C1 C2 C3 C4 D
PERE MJ 1.63E+01 4.11E-03 8.36E-01 0 2.3E-04 9.78E-02 0 -1.49E+01
PERM MJ 9.02E-01 0 -8.3E-01 0 0 -7.2E-02 0 0
PERT MJ 1.72E+01 4.11E-03 5.63E-03 0 2.3E-04 2.58E-02 0 -1.49E+01
PENRE MJ 1.19E+02 1.29E+00 3.1E-02 0 7.3E-02 1.2E-01 0 -3.43E+01
PENRM MJ 1.95E-02 0 0 0 0 -1.95E-02 0 0
PENRT MJ 1.19E+02 1.29E+00 3.1E-02 0 7.3E-02 1E-01 0 -3.43E+01
SM kg 7.18E-01 0 0 0 0 0 0 0
RSF MJ 0 0 0 0 0 0 0 0
NRSF MJ 0 0 0 0 0 0 0 0
FW m3 5.71E-02 7.42E-06 2.86E-04 0 4.12E-07 5.42E-04 0 -2.64E-02
PERE = Use of renewable primary energy excluding renewable primary energy resources used as raw materials; PERM = Use of renewable primary
energy resources used as raw materials; PERT = Total use of renewable primary energy resources; PENRE = Use of non-renewable primary energy
excluding non-renewable primary energy resources used as raw materials; PENRM = Use of non-renewable primary energy resources used as raw
materials; PENRT = Total use of non-renewable primary energy resources; SM = Use of secondary material; RSF = Use of renewable secondary fuels;
NRSF = Use of non-renewable secondary fuels; FW = Use of net fresh water
RESULTS OF THE LCA – WASTE CATEGORIES AND OUTPUT FLOWS according to EN 15804+A2:
1 piece TS Compakt
Parameter Unit A1-A3 A4 A5 C1 C2 C3 C4 D
HWD kg 1.68E-07 1.25E-10 4.57E-11 0 7.08E-12 3.74E-10 0 -2.76E-07
NHWD kg 1.36E+00 1.31E-04 3.07E-03 0 7.46E-06 2.2E-02 0 -5.47E-01
RWD kg 1.72E-03 1.4E-06 1.63E-06 0 7.83E-08 3.76E-06 0 -3.61E-03
CRU kg 0 0 0 0 0 0 0 0
MFR kg 0 0 0 0 0 1.14E+00 0 0
MER kg 0 0 0 0 0 0 0 0
EEE MJ 0 0 1.48E-01 0 0 4.06E-01 0 0
EET MJ 0 0 2.69E-01 0 0 9.24E-01 0 0
4 Environmental Product Declaration - dormakaba - Door closer TS Compakt
HWD = Hazardous waste disposed; NHWD = Non-hazardous waste disposed; RWD = Radioactive waste disposed; CRU = Components for re-use;
MFR = Materials for recycling; MER = Materials for energy recovery; EEE = Exported electrical energy; EET = Exported thermal energy
RESULTS OF THE LCA – additional impact categories according to EN 15804+A2-optional:
1 piece TS Compakt
Parameter Unit A1-A3 A4 A5 C1 C2 C3 C4 D
Disease
PM 1.38E-06 2.7E-08 1.52E-10 0 2.7E-11 4.87E-10 0 -1.4E-07
incidence
IR kBq U235 eq 1.97E-01 2.01E-04 2.52E-04 0 1.12E-05 3.48E-04 0 -7.19E-01
ETP-fw CTUe 3.96E+01 9.09E-01 1.47E-02 0 5.17E-02 3.77E-02 0 -1.21E+01
HTP-c CTUh 3.94E-09 1.71E-11 7.77E-13 0 9.72E-13 3.24E-12 0 -2.91E-10
HTP-nc CTUh 1.28E-07 7.65E-10 3.37E-11 0 4.16E-11 3.24E-10 0 7.08E-09
SQP SQP 2.31E+01 3.35E-03 8.21E-03 0 1.87E-04 2.99E-02 0 -1.12E+00
PM = Potential incidence of disease due to PM emissions; IR = Potential Human exposure efficiency relative to U235; ETP-fw = Potential comparative
Toxic Unit for ecosystems; HTP-c = Potential comparative Toxic Unit for humans (cancerogenic); HTP-nc = Potential comparative Toxic Unit for humans
(not cancerogenic); SQP = Potential soil quality index
Disclaimer 1 – for the indicator “Potential Human exposure efficiency relative to U235”. This impact category deals mainly with the
eventual impact of low-dose ionizing radiation on human health of the nuclear fuel cycle. It does not consider effects due to possible
nuclear accidents, occupational exposure or radioactive waste disposal in underground facilities. Potential ionizing radiation from the
soil, radon and from some construction materials is also not measured by this indicator.
Disclaimer 2 – for the indicators “abiotic depletion potential for non-fossil resources”, “abiotic depletion potential for fossil resources”,
“water (user) deprivation potential, deprivation-weighted water consumption”, “potential comparative toxic unit for ecosystems”,
“potential comparative toxic unit for humans – cancerogenic”, “Potential comparative toxic unit for humans - not cancerogenic”,
“potential soil quality index”. The results of this environmental impact indicator shall be used with care as the uncertainties on these
results are high as there is limited experience with the indicator.
This EPD was created using a software tool.
References
EN 1634-1 Standard for Positive Pressure Fire Tests of Door Assemblies
EN 1634-1:2018-04; Fire resistance and smoke control tests
fordoor and shutter assemblies, openable windows and Further References
elements of building hardware - Part 1: Fire resistance test for
door andshutter assemblies and openable windows IBU 2021
General Instructions for the EPD programme of Institut Bauen
UL 10C:3EDUL 10C:3ED; 2016-06-09 und Umwelt e.V. Version 2.0, Berlin: Institut Bauen und Umwelt
Positive Pressure Fire Tests of Door Assemblies e.V., 2021. www.ibu-epd.com
EN 15804 GaBi ts software
EN 15804+A2:2019+AC:2021, Sphera Solutions GmbH
Sustainability of construction works — Environmental Product Gabi Software System and Database for Life Cycle Engineering
Declarations — Core rules for the product category of 19922020
construction products Version 10.0.0.71
University of Stuttgart
EN 1634-1 Leinfelden-Echterdingen
EN 1634-1:2018-04, Fire resistance and smoke control tests for
door and shutter assemblies, openable windows and elements GaBi ts documentation
of building hardware - Part 1: Fire resistance test for door and GaBi life cycle inventory data documentation
shutter assemblies and openable windows. (https://www.gabisoftware.com/support/gabi/gabidatabase-
2020-lcidocumentation/).
ECHA
European Chemical Agency LCA-tool dormakaba
Tool No.: IBU-DOR-202104-LT1-EN
ISO 14025 Developed by Sphera Solutions GmbH
DIN EN ISO 14025:201110, Environmental labels and
declarations — Type III environmental declarations — PCR Part A
Principles and procedures PCR – Part A: Calculation Rules for the Life Cycle Assessment
and Requirements on the Project Re-port according to EN
REACH 15804+A2:2019,
Regulation (EC) No 1907/2006 of the European Parliament and Version 1.0, 2020, Institut Bauen und Umwelt e.V., www.ibu-
of the Council on the Registration, Evaluation, Authorisation epd.com.
and Restriction of Chemicals (REACH)
PCR Part B
RoHS PCR – Part B: Requirements on the EPD for Building Hardware
2011/65/EU, Directive on the restriction of the use of certain product, version 08/2021, Institut Bauen und Umwelt e.V.,
hazardous substances in electrical and electronic equipment www.ibu-epd.com.
UL 10c
5 Environmental Product Declaration - dormakaba - Door closer TS Compakt
6 Environmental Product Declaration - dormakaba - Door closer TS Compakt
Publisher
Institut Bauen und Umwelt e.V. +49 (0)30 3087748- 0
Hegelplatz 1 info@ibu-epd.com
10117 Berlin www.ibu-epd.com
Germany
Programme holder
Institut Bauen und Umwelt e.V. +49 (0)30 3087748- 0
Hegelplatz 1 info@ibu-epd.com
10117 Berlin www.ibu-epd.com
Germany
Author of the Life Cycle Assessment
dormakaba International Holding GmbH +49 2333 793-0
DORMA Platz 1 info.de@dormakaba.com
58256 Ennepetal www.dormakaba.com
Germany
Owner of the Declaration
dormakaba International Holding GmbH +49 2333 793-0
DORMA Platz 1 info.de@dormakaba.com
58256 Ennepetal www.dormakaba.com
Germany
7 Environmental Product Declaration - dormakaba - Door closer TS Compakt
