ENVIRONMENTAL PRODUCT DECLARATION
as per ISO 14025 and EN 15804+A2
Owner of the Declaration VELUX Group
Publisher Institut Bauen und Umwelt e.V. (IBU)
Programme holder Institut Bauen und Umwelt e.V. (IBU)
Declaration number EPD-VEL-20220033-CBE4-EN
Issue date 24.05.2022
Valid to 23.05.2027
VELUX PUR roof windows (triple glazing configuration)
VELUX Group
www.ibu-epd.com | https://epd-online.com
General Information
VELUX Group VELUX PUR roof windows (triple glazing
configuration)
Programme holder Owner of the declaration
IBU – Institut Bauen und Umwelt e.V. VELUX Group
Hegelplatz 1 Ådalsvej 99
10117 Berlin 2970 Hørsholm
Germany Denmark
Declaration number Declared product / declared unit
EPD-VEL-20220033-CBE4-EN The declared unit is a PUR roof window of one square meter (m2) with
triple glazing configuration.
The declared unit is based on the configuration of a standard size window
measuring 1.23 m * 1.48 m.
This declaration is based on the product category rules: Scope:
Windows and doors , 01.08.2021 The EPD is a representative EPD covering VELUX PUR roof windows as
(PCR checked and approved by the SVR) specified in more detail in the product description. The products are
manufactured by the VELUX Group at production sites in different
locations in Europe for sale throughout Europe.
Issue date The owner of the declaration shall be liable for the underlying information
and evidence; the IBU shall not be liable with respect to manufacturer
24.05.2022
information, life cycle assessment data and evidences.
The EPD was created according to the specifications of EN 15804+A2. In
Valid to
the following, the standard will be simplified as EN 15804.
23.05.2027
Verification
The standard EN 15804 serves as the core PCR
Independent verification of the declaration and data according to ISO
14025:2011
internally X externally
Dipl.-Ing. Hans Peters
(Chairman of Institut Bauen und Umwelt e.V.)
Florian Pronold Juliane Franze,
(Managing Director Institut Bauen und Umwelt e.V.) (Independent verifier)
1 Environmental Product Declaration - VELUX Group - VELUX PUR roof windows (triple glazing configuration)
Product
window type.
Product description/Product definition
The VELUX polyurethane (PUR) roof windows are skylight The glass panes are with triple glazing and different glass
window products for sale in the European market. The product configurations are covered by the EPD. The glass thickness
family covers a range of product varieties as specified in the ranges from 10 to 13 mm. The glass panes have cavities filled
table on page 3. All the windows have a PUR frame/sash with a with Krypton or Argon gas. The EPD is based on an average of
wooden core. Some windows can be opened (venting), while the included glazing unit configurations.
others cannot be opened (fixed). Some of the window varieties
can be used in conjunction with electronic devices for automatic Only the window modules are included, which means that any
opening and closing, while other windows are opened and applied electronics, additional equipment, engines etc. are not
closed manually. The calculations are based on the part of the EPD.
representative window type named GPU. In the LCA, the GPU
was assessed to be a conservative choice for a representative
2 Environmental Product Declaration - VELUX Group - VELUX PUR roof windows (triple glazing configuration)
For the placing on the market of the product in the European Name Value Unit
Union/European Free Trade Association (EU/EFTA) (with the
Fire resistance class § 4.4.1 D-s2.d2 class
exception of Switzerland) Regulation (EU) No. 305/2011 (CPR)
Air permeability , § 4.14 4 class
applies. The product needs a declaration of performance taking
Resistance to wind load, §
into consideration EN 14351-1:2006+A2:2016, Windows and
4.2 (for window width >1140
doors - Product standard, performance characteristics - Part 1: C3 class
mm or height > 1398 mm no
Windows and external pedestrian doorsets. For the application
performance is determined)
and use, the respective national provisions apply.
4 mm toughened - 13
Application Resistance to snow loads, § mm - 3 mm heat
mm
VELUX PUR roof windows are used in renovation and new 4.3 strengthened - 13 mm -
build. Either installed as a single window or in a combination of 6.8 mm laminated float
multiple windows. Watertightness, § 4.5 E900 class
Impact resistance, § 4.7 (for
Technical Data
window width <550 mm or
The Declaration of Performance including relevant technical 3 class
height <778 mm no
specifications and test methods/test standards can be
performance is determined)
downloaded from the website www.velux.com/ce.
Load-bearing capacity of
test is passed -
The performance values are specific for each PUR roof window safety devices, § 4.8
variant covered by the EPD. Acoustic performance, §
37 (-2; -4) -
4.11
The declared values in the table relate to the reference product Thermal transmittance, §
incl. an average pane. For other covered product variants, 4.12 , 90 degree installation 1,0 W/(m2K)
specific values can be selected at the bottom of the above- acc. to EN 10077-1/2
mentioned download page.
Solar factor, § 4.13 0.44 -
Constructional data (Reference product GPU incl. pane Light transmittance, § 4.13 0.62 -
variant 66. For other variation, see velux.com/ce)
Product performance data in accordance with DS/EN 14351-
1:2006+A2:2016, Windows and doors - Product standard,
performance characteristics - Part 1: Windows and external
pedestrian doorsets.
Base materials/Ancillary materials
Name Value Unit
Glazing unit 55 %
PUR/wooden frame 23 %
Galvanized steel components 17 %
Other materials 5 %
This product/article/at least one partial article contains
substances listed in the candidate list (date:
07.03.2022) exceeding 0.1 percentage by mass: NO.
Recycled content
The values stated in the table relate to the recycled material
streams in VELUX production.
3 Environmental Product Declaration - VELUX Group - VELUX PUR roof windows (triple glazing configuration)
because the use stage modules are not included in the EPD.
Reference service life
No reference service life (RSL) is defined for the roof windows
LCA: Calculation rules
profiles, drilling of holes, clamping and glueing,
Declared Unit mounting of gaskets, brackets, panes etc. as well as
Multiple product dimensions are represented by this EPD as stacking on pallets.
specified in the product description.
The declared unit is 1 m2 window calculated based on one End of life stage:
representative window module measuring 1.23 m * 1.48 m
• C1 - De-construction/demolition: de-construction of the
(reference window based on EN 14351-1) with triple glazed
window with the use of an electric screwdriver
window panes.
• C2 - Transport: transport of window materials to
Declared unit
incineration and recycling
Name Value Unit
• C3 - Waste processing: sorting of glass waste,
conversion factor 50 -
incineration of plastic and rubber parts
Declared unit 1 m2
• C4 - Disposal: disposal of all materials
A data quality and a sensitivity analysis shows that the results
are robust with regards to data quality and appropriateness.
There is low variability of production processes and product Benefits and loads beyond the system boundaries:
variations have a limited influence on the results. • D - Reuse, recovery and recycling potential: benefits
from plastic incineration processes and material
System boundary
recycling of metal and glass.
Type of EPD: Cradle to gate - with options. The following life
cycle phases were considered: Geographic Representativeness
Product stage: Land or region, in which the declared product system is
• A1 - Raw material supply: extraction and processing, manufactured, used or handled at the end of the product´s
production of the pre-products (e.g. laminated glass, lifespan: Europe
brackets, sealant...) and packaging components
(primarily cardboard)
Comparability
• A2 - Transport:
Basically, a comparison or an evaluation of EPD data is only
Transport of pre-products and packaging components to
possible if all the data sets to be compared were created
the manufacturing sites
according to EN 15804 and the building context, respectively
• A3 - Manufacturing: The PUR profiles and the panes are the product-specific characteristics of performance, are taken
produced internally at VELUX production sites. into account.
Subsequently, the final production and assembly of the
windows take place, which involves shortening of
LCA: Scenarios and additional technical information
Characteristic product properties of biogenic carbon
End of life (C1-C4)
6.9 kg of wood is used in the core window frames and 3.1 kg of
cardboard packaging is used per declared unit. Name Value Unit
Collected as mixed construction waste 50 kg
Information describing the biogenic Carbon Content at
factory gate Recycling 18 kg
Name ValueUnit Energy recovery 13 kg
kg Landfilling 19 kg
Biogenic carbon content in product 3.6
C
Reuse, recovery and/or recycling potentials (D), relevant
Biogenic carbon content in accompanying kg
2.5 scenario information
packaging C
The recycling efficiency for all materials is maximum 90 % in
Note: 1 kg of biogenic carbon is equivalent to 44/12 kg of CO . accordance with EN 17213. This means that only 90 % of the
2
recycled materials substitute primary materials. Secondary
materials in the windows do not substitute primary materials in
The construction process stage and the use stage modules are the end-of-life scenario. The recycled glass is used as container
not declared. However, the quantity of packaging generated in glass in the end-of-life scenario.
module A5 is declared as scenario information. Name Value Unit
Installation into the building (A5) Glass recycled 30 %
Name ValueUnit Metal recycled 95 %
Cardboard packaging for waste treatment 3.1 kg Plastic incinerated with energy recovery 95 %
Plastic packaging (primarily EPS) for waste
0.3 kg
treatment
4 Environmental Product Declaration - VELUX Group - VELUX PUR roof windows (triple glazing configuration)
LCA: Results
DESCRIPTION OF THE SYSTEM BOUNDARY (X = INCLUDED IN LCA; MND = MODULE OR INDICATOR NOT DECLARED; MNR
= MODULE NOT RELEVANT)
Benefits and
Construction loads beyond
Product stage Use stage End of life stage
process stage the system
boundaries
la ire ta m w a Ry lp p u s tro p s n a rT g n iru tc a fu n a M e h t m o rf tro p s n a rTe tis e h t o t e ta g y lb m e s s A e s U e c n a n e tn ia M ria p e R tn e m e c a lp e R tn e m h s ib ru fe R y g re n e la n o ita re p Oe s u re ta w la n o ita re p Oe s u n o itc u rts n o c -e Dn o itilo m e d tro p s n a rT g n is s e c o rp e ts a W la s o p s iD -e s u e R-y re v o c e R-g n ilc y c e Rla itn e to p
A1 A2 A3 A4 A5 B1 B2 B3 B4 B5 B6 B7 C1 C2 C3 C4 D
X X X MND MND MND MND MNR MNR MNR MND MND X X X X X
RESULTS OF THE LCA - ENVIRONMENTAL IMPACT according to EN 15804+A2: 1 m2 Roof windows with triple glazing
Parameter Unit A1 A2 A3 C1 C2 C3 C4 D
GWP-total kg CO 2 eq 1.27E+02 3.37E+00 1.57E+01 1.84E-03 1.49E-01 2.73E+01 1.14E+00 -3.87E+01
GWP-fossil kg CO 2 eq 1.45E+02 3.34E+00 1.31E+01 1.82E-03 1.48E-01 1.5E+01 3.82E-01 -3.86E+01
GWP-biogenic kg CO 2 eq -1.87E+01 -4.26E-03 2.52E+00 1.55E-05 -1.89E-04 1.24E+01 7.52E-01 -6.88E-02
GWP-luluc kg CO 2 eq 1.03E-01 2.73E-02 1.85E-02 2.58E-06 1.21E-03 6.33E-04 1.29E-03 -1.46E-02
ODP kg CFC11 eq 2.97E-06 4.26E-16 6.46E-11 4.36E-17 1.89E-17 7.26E-09 1.19E-15 -1.07E-13
AP mol H+ eq 5.47E-01 1.07E-02 3.94E-02 3.79E-06 4.77E-04 4.99E-03 2.35E-03 -1.33E-01
EP-freshwater kg P eq 8.33E-03 9.91E-06 1.36E-04 4.88E-09 4.4E-07 1.81E-05 7.3E-06 -2.44E-05
EP-marine kg N eq 1.05E-01 4.96E-03 1.25E-02 9E-07 2.2E-04 1.76E-03 6.68E-04 -2.81E-02
EP-terrestrial mol N eq 1.18E+00 5.54E-02 1.27E-01 9.44E-06 2.46E-03 2.42E-02 7.23E-03 -3.11E-01
kg NMVOC
POCP 3.25E-01 9.67E-03 3.41E-02 2.44E-06 4.29E-04 4.77E-03 2.12E-03 -7.57E-02
eq
ADPE kg Sb eq 2.39E-03 2.54E-07 3.88E-06 5.35E-10 1.13E-08 2.78E-07 3.35E-08 -2.39E-05
ADPF MJ 2.18E+03 4.44E+01 2.03E+02 3.24E-02 1.97E+00 8.71E+00 5.13E+00 -4.93E+02
m3 world eq
WDP 1.29E+01 2.9E-02 1.25E+00 2.92E-04 1.29E-03 2.82E+00 3.19E-02 -2.56E+00
deprived
GWP = Global warming potential; ODP = Depletion potential of the stratospheric ozone layer; AP = Acidification potential of land and water; EP =
Eutrophication potential; POCP = Formation potential of tropospheric ozone photochemical oxidants; ADPE = Abiotic depletion potential for non-fossil
resources; ADPF = Abiotic depletion potential for fossil resources; WDP = Water (user) deprivation potential)
RESULTS OF THE LCA - INDICATORS TO DESCRIBE RESOURCE USE according to EN 15804+A2: 1 m2 Roof windows with
triple glazing
Parameter Unit A1 A2 A3 C1 C2 C3 C4 D
PERE MJ 2.34E+02 2.48E+00 1.04E+02 1.49E-02 1.1E-01 1.15E+02 5.82E-01 -9.49E+01
PERM MJ 1.22E+02 0 6.21E+01 0 0 -1.14E+02 0 0
PERT MJ 3.55E+02 2.48E+00 1.66E+02 1.49E-02 1.1E-01 1.67E+00 5.82E-01 -9.49E+01
PENRE MJ 1.98E+03 4.45E+01 1.89E+02 3.24E-02 1.97E+00 1.48E+02 5.13E+00 -4.94E+02
PENRM MJ 2.08E+02 0 1.44E+01 0 0 -1.4E+02 0 0
PENRT MJ 2.19E+03 4.45E+01 2.03E+02 3.24E-02 1.97E+00 8.71E+00 5.13E+00 -4.94E+02
SM kg 6.54E+00 0 1.37E-03 0 0 0 0 0
RSF MJ 0 0 0 0 0 0 0 0
NRSF MJ 0 0 0 0 0 0 0 0
FW m3 6.97E-01 2.84E-03 7.95E-02 1.45E-05 1.26E-04 6.66E-02 1.01E-03 -2.05E-01
PERE = Use of renewable primary energy excluding renewable primary energy resources used as raw materials; PERM = Use of renewable primary
energy resources used as raw materials; PERT = Total use of renewable primary energy resources; PENRE = Use of non-renewable primary energy
excluding non-renewable primary energy resources used as raw materials; PENRM = Use of non-renewable primary energy resources used as raw
materials; PENRT = Total use of non-renewable primary energy resources; SM = Use of secondary material; RSF = Use of renewable secondary fuels;
NRSF = Use of non-renewable secondary fuels; FW = Use of net fresh water
RESULTS OF THE LCA – WASTE CATEGORIES AND OUTPUT FLOWS according to EN 15804+A2:
1 m2 Roof windows with triple glazing
Parameter Unit A1 A2 A3 C1 C2 C3 C4 D
HWD kg 3.87E-03 2.24E-09 2.73E-04 8.56E-12 9.95E-11 1.45E-09 5.63E-10 -6.01E-08
NHWD kg 5.72E+00 6.61E-03 5.03E-01 2.3E-05 2.93E-04 2.03E+01 1.85E+01 -3.41E+00
RWD kg 3.72E-02 5.38E-05 1.61E-02 4.82E-06 2.39E-06 3.5E-04 4.78E-05 -2.19E-02
CRU kg 0 0 0 0 0 0 0 0
MFR kg 2.89E-02 0 2E+00 0 0 1.77E+01 0 0
MER kg 0 0 0 0 0 1.27E+01 0 0
EEE MJ 4.13E-02 0 0 0 0 0 0 4.99E+01
EET MJ 6.03E-02 0 0 0 0 0 0 9.07E+01
5 Environmental Product Declaration - VELUX Group - VELUX PUR roof windows (triple glazing configuration)
HWD = Hazardous waste disposed; NHWD = Non-hazardous waste disposed; RWD = Radioactive waste disposed; CRU = Components for re-use;
MFR = Materials for recycling; MER = Materials for energy recovery; EEE = Exported electrical energy; EET = Exported thermal energy
RESULTS OF THE LCA – additional impact categories according to EN 15804+A2-optional:
1 m2 Roof windows with triple glazing
Parameter Unit A1 A2 A3 C1 C2 C3 C4 D
Disease
PM 6.38E-06 5.8E-08 4.5E-07 3.19E-11 2.58E-09 3.94E-08 2.72E-08 -1.3E-06
incidence
IR kBq U235 eq 8.49E+00 7.7E-03 1.9E+00 7.91E-04 3.42E-04 5.93E-02 5.42E-03 -3.98E+00
ETP-fw CTUe 2.34E+03 3.21E+01 1.22E+02 1.36E-02 1.43E+00 5.2E+00 3.51E+00 -2.03E+02
HTP-c CTUh 1.68E-06 6.48E-10 6.14E-09 3.86E-13 2.88E-11 2.98E-10 3.46E-10 -2.76E-08
HTP-nc CTUh 2.56E-06 3.81E-08 5.52E-07 1.45E-11 1.69E-09 2.3E-08 3.76E-08 -3.04E-07
SQP SQP 1.57E+03 1.53E+01 8.34E+02 1.02E-02 6.77E-01 3.05E+00 1.03E+00 -3.44E+01
PM = Potential incidence of disease due to PM emissions; IR = Potential Human exposure efficiency relative to U235; ETP-fw = Potential comparative
Toxic Unit for ecosystems; HTP-c = Potential comparative Toxic Unit for humans (cancerogenic); HTP-nc = Potential comparative Toxic Unit for humans
(not cancerogenic); SQP = Potential soil quality index
Disclaimer 1 – for the indicator IRP. This impact category deals mainly with the eventual impact of low dose ionizing radiation on human
health of the nuclear fuel cycle. It does not consider effects due to possible nuclear accidents, occupational exposure or radioactive
waste disposal in underground facilities. Potential ionizing radiation from the soil, radon and (from) some construction materials is also
not measured by this indicator.
Disclaimer 2 – for the indicators ADPE, ADPF, WDP, ETP-fw, HTP-c, HTP-nc, SQP. The results of this environmental impact indicator
shall be used with care as the uncertainties on these results are high or as there is limited experience with the indicator.
References
IBU PCR Part A Windows and external pedestrian doorsets.
IBU PCR Part A: Institut Bauen und Umwelt e.V., Product
Category Rules for Building-Related Products and Services. EN 15804
Calculation Rules for the Life Cycle Assessment and EN 15804+A2+AC:2021, Sustainability of construction works -
Requirements on the Project Report according to EN Environmental Product Declarations - Core rules for the product
15804+A2:2019. category of construction products.
IBU PCR Part B EN 17213
IBU PCR Part B: Institut Bauen und Umwelt e.V., Requirements EN 17213:2020, Windows and doors – Environmental Product
on the EPD for Windows and doors, version 1.4: 2021. Declarations – Product category rules for windows and
pedestrian doorsets.
IBU 2021
IBU 2021 Institut Bauen und Umwelt e.V.: General Instructions ECHA Candidate list
for the EPD programme of Institut Bauen und Umwelt e.V. EHCA Candidate list of substances of very high concern: status
Version 2.0, Berlin: Institut Bauen und Umwelt e.V., 2021. 07.03.2022
www.ibu-epd.com.
ISO 10077-1
EN 13501-1 ISO 10077-1:2017, Thermal performance of windows, doors
EN 13501-1 EN13501-1, 2018: Fire classification of and shutters - Calculation of thermal transmittance - Part 1:
construction products and building elements - Part 1: General.
Classification using data from reaction to fire tests.
ISO 10077-2
ISO 14025 ISO 10077-2:2017, Thermal performance of windows, doors
DIN EN ISO 14025:2011-10, Environmental labels and and shutters - Calculation of thermal transmittance - Part 2:
declarations - Type III environmental declarations - Principles Numerical method for frames.
and procedures.
GaBi LCA software and database
EN 14351-1 The LCA modelling software is GaBi program version 9.5.2.49
EN 14351-1:2006+A2:2016, Windows and doors - Product with corresponding databases from Sphera Solutions GmbH.
standard, performance characteristics - Part 1: Documentation hyperlink www.gabi-software.com/support/gabi.
6 Environmental Product Declaration - VELUX Group - VELUX PUR roof windows (triple glazing configuration)
Publisher
Institut Bauen und Umwelt e.V. +49 (0)30 3087748- 0
Hegelplatz 1 info@ibu-epd.com
10117 Berlin www.ibu-epd.com
Germany
Programme holder
Institut Bauen und Umwelt e.V. +49 (0)30 3087748- 0
Hegelplatz 1 info@ibu-epd.com
10117 Berlin www.ibu-epd.com
Germany
Author of the Life Cycle Assessment
FORCE Technology +4543250856
Park Alle 345 chme@force.dk
2605 Brøndby www.forcetechnology.com
Denmark
Owner of the Declaration
VELUX Group +4545164726
Ådalsvej 99 jakob.roerbech@velux.com
2970 Hørsholm www.velux.com
Denmark
7 Environmental Product Declaration - VELUX Group - VELUX PUR roof windows (triple glazing configuration)
