ENVIRONMENTAL PRODUCT DECLARATION
as per ISO 14025 and EN 15804+A2
Owner of the Declaration Sika Corporation
Publisher Institut Bauen und Umwelt e.V. (IBU)
Programme holder Institut Bauen und Umwelt e.V. (IBU)
Declaration number EPD-SIK-20230176-CBA2-EN
Issue date 22/06/2023
Valid to 21/06/2028
Sika ViscoCrete®-2100
Sika
www.ibu-epd.com | https://epd-online.com
General Information
Sika Sika ViscoCrete®-2100
Programme holder Owner of the declaration
IBU – Institut Bauen und Umwelt e.V. Sika Corporation
Hegelplatz 1 Polito Avenue 201
10117 Berlin 07071 Lyndhurst, NJ
Germany United States
Declaration number Declared product / declared unit
EPD-SIK-20230176-CBA2-EN 1kg of Sika ViscoCrete®-2100 with a density of 1.08 g/ml
This declaration is based on the product category rules: Scope:
Concrete admixtures, 06/04/2023 This core-EPD relates to 1kg of Sika ViscoCrete®-2100 (admixture group
(PCR checked and approved by the SVR) of superplasticizer) applied into the building, manufactured at Sika's plant
in Fairless Hills, Pennsylvania 19030, United States and is representative
for the year 2021.
Issue date The results in this core-EPD were calculated using an LCA-tool verified by
IBU in 2023.
22/06/2023
The owner of the declaration shall be liable for the underlying information
and evidence; the IBU shall not be liable with respect to manufacturer
information, life cycle assessment data and evidences.
Valid to
21/06/2028 The EPD was created according to the specifications of EN 15804+A2. In
the following, the standard will be simplified as EN 15804.
Verification
The standard EN 15804 serves as the core PCR
Independent verification of the declaration and data according to ISO
14025:2011
internally X externally
Dipl.-Ing. Hans Peters
(Chairman of Institut Bauen und Umwelt e.V.)
Florian Pronold Matthias Schulz,
(Managing Director Institut Bauen und Umwelt e.V.) (Independent verifier)
1 Environmental Product Declaration - Sika - Sika ViscoCrete®-2100
Product
• Type A: at 3 days 126%, at 7 days 125%, at 28 days
Product description/Product definition
111%, at 90 days 109%, at 6 months 111%, and at 1
Sika ViscoCrete®-2100 is a high range water reducing
year 112%
admixture utilizing Sika's ViscoCrete polycarboxylate
• Type F: at 1 day 190%, at 3 days 160%, at 7 days
technology. Sika ViscoCrete®-2100 meets the requirements of
151%, at 28 days 131%, at 90 days 134%, at 6 months
ASTM C494/AASHTO M 194, Type A & F.
141% and at 1 year 141%
Sika ViscoCrete®-2100 is designed for use in both ready mix
and precast applications whenever high plasticity and
Additional technical data are not relevant for the US market.
increased early/ultimate strengths are required. Sika
ViscoCrete®-2100 can be used for production of SCC (Self
Performance data of the product in accordance with the
Consolidating Concrete), UHPC (Ultra High-Performance
declaration of performance with respect to its essential
Concrete) as well as for production of conventional slump
characteristics according to EN 934-2:2009+A1:2012,
concrete.
Admixtures for concrete, mortar and grout – Part 2: Concrete
This additive considerably reduces the water content of mixed
admixtures – Definitions, requirements, conformity, marking and
concrete without detriment to its consistency or enhances its
labelling.
slump with or without change to the water content.
For the purposes of this EPD, Sika's Fairless Hills, Base materials/Ancillary materials
Pennsylvania 19030 manufacturing site was selected.
The raw materials and additives of Sika ViscoCrete®-2100 can
The product needs a declaration of performance taking into
be given as follows:
consideration EN 934-2+A1, Admixtures for concrete, mortar
and grout – Part 2: Concrete admixtures – Definitions, • Water: 60 – 70%
requirements, conformity, marking and labelling and the CE- • Polycarboxylate: 30 – 45%
marking. For the application and use the respective national • Additives: 0.5 - 5%
provisions apply. Sika ViscoCrete®-2100 is non-hazardous under the criteria of
the Federal OSHA Hazard Communication Standard 29CFR
Application 1910.1200. It does not contain any substances that OSHA
Sika ViscoCrete®-2100 is used as a constituent material to regulates as carcinogens or potential carcinogens, according to
produce concrete. It can be used in combination with other Sika Federal OSHA Hazard Communication Standard 29CFR
admixtures and can be successfully used in mix designs 1910.1003, in concentrations of 0.1% or greater.
utilizing supplementary cementitious materials. Sika ViscoCrete®-2100 is a non-chloride-based admixture, it
does not contain any intentionally added chlorides.
Technical Data In particular:
Sika ViscoCrete®-2100 meets the requirements of ASTM
• This product contains substances listed in the candidate
C494/AASHTO M 194, Type A & F.
list (date: 20.04.2023) exceeding 0.1 percentage by
Constructional data mass: No
Name Value Unit • This product contains other CMR substances in
categories 1A or 1B which are not on the candidate list,
40.00 ±
Solid Content (ASTM C494) % exceeding 0.1 percentage by mass: No
4.80
• Biocide products were added to this construction
pH (ASTM E70) 4.30 ± 2.00 -
product orit has been treated with biocide products (this
1.080 ± then concerns a treated product as defined by the (EU)
Specific Gravity (ASTM C494) g/cm3
0.010 Ordinance on Biocide Products No. 528/2012): No
Chloride Content (EN 480-10) <500 ppm
Air content of fresh concrete (ASTM C494)
6.7 %
Type A & F
Reference service life
Water reduction (ASTM C494) Type A 6 %
The durability of concrete admixtures is normally at least as
Water reduction (ASTM C494) Type F 13 % long as the lifetime of the building in which it is used. The
Intial setting time (ASTM C494) Type A + 0:04 hr:min experimental data show that the reference life is greater than
Intial setting time (ASTM C494) Type F - 0:06 hr:min 50 years.
The documentation of the RSL is not required for the EPDs
Final setting time (ASTM C494) Type A + 0:01 hr:min
calculated using the EPD tool from Sika since the entire life
Final setting time (ASTM C494) Type F - 0:10 hr:min
cycle is not declared. Only modules A1-A3, A4, A5, C1-C4 and
Compressive strength (ASTM C494): D are considered.
LCA: Calculation rules
Name Value Unit
Declared Unit
Declared unit 1 kg
The EPD refers to the declared unit of 1kg of concrete
admixture (superplasticizer) applied into the building with a
Gross density 1080 kg/m3
density of 1.08 g/ml in accordance with IBU PCR 04-2023 part .
B for concrete admixtures.
System boundary
Declared unit and mass reference
Declaration type with respect to life cycle stages covered
according to clause 5.2 EN 15804+A2 is cradle to gate with
modules C1–C4 and module D (A1–A3, A4, A5, C and D).
2 Environmental Product Declaration - Sika - Sika ViscoCrete®-2100
Modules taken into account:
• 100% disposal (C4), modelled by landfill process where
• A1 Production of preliminary products admixtures end their life cycle.
• A2 Transport to the plant Module D accounts for benefits that are beyond the defined
• A3 Production including provision of energy, production system boundaries. Credits are generated during the
of auxiliaries and consumables and waste treatment incineration of the installation scrap in module A5.
• A4 Transport from the construction site to the installation
site Geographic Representativeness
• A5 Installation, admixtures applied into the building Land or region, in which the declared product system is
during A5 phase operations. At this stage, an impact of manufactured, used or handled at the end of the product´s
the production and treatment of installation residue lifespan: United States
equal to 1% of the product is considered.
• C1-C2-C4-D
Comparability
The building deconstruction (demolition process) takes place in
Basically, a comparison or an evaluation of EPD data is only
C1 module which considers energy production and
possible if all the data sets to be compared were created
consumption in terms of diesel and all the emissions connected
according to EN 15804 and the building context, respectively
with the fuel-burning process. After the demolition, the
the product-specific characteristics of performance, are taken
admixture is transported to the end-of-life processing (C2
into account.
module) where all the impacts related to the transport
Sphera LCA for Expert software (former GaBi) (version 10) and
processes are considered.
Managed LCA Content (2022.2) have been used.
One scenario is considered for the final treatment of the waste:
LCA: Scenarios and additional technical information
Material loss regards the amount of product not used during the
Characteristic product properties of biogenic carbon application phase into the building. This amount is 1 % of the
No biogenic carbon is contained in the product. Since the product, impacts related to the production of this part are
product is delivered to the installation site in tank trucks, no charged to the A5 module. This percentage is considered as
packaging is considered. waste to incineration since the product has a calorific value and
Information on describing the biogenic Carbon Content at impacts of its end of life have been considered in the LCA
factory gate model and declared in A5.
Name ValueUnit
.
kg
Biogenic carbon content in product - End of life (C1-C4)
C
C1: This module considers the use of machinery (7.5E-5 kg of
Biogenic carbon content in accompanying kg
- diesel for kg handled) to dismantle the product to enable its
packaging C
subsequent transport.
C2: The concrete demolition waste is transported from the
. building site to a treatment plant or disposal site by truck and
an average distance of 50 km is considered.
Transport from the gate to the side (A4)
C4: The results for the end-of-life are declared for one scenario:
Name Value Unit
Name Value Unit
Transport distance 5000 km
Landfill percentage 100 %
Gross weight 34-40 t
Material to landfill 1 kg
Payload capacity 27 t
Assembly (A5)
Name Value Unit
Material loss 0.01 kg
Other resources - kg
3 Environmental Product Declaration - Sika - Sika ViscoCrete®-2100
LCA: Results
.
DESCRIPTION OF THE SYSTEM BOUNDARY (X = INCLUDED IN LCA; ND = MODULE OR INDICATOR NOT DECLARED; MNR =
MODULE NOT RELEVANT)
Benefits and
Construction loads beyond
Product stage Use stage End-of-life stage
process stage the system
boundaries
la ire ta m w a Ry lp p u s tro p s n a rT g n iru tc a fu n a M e h t m o rf tro p s n a rTe tis e h t o t e ta g y lb m e s s A e s U e c n a n e tn ia M ria p e R tn e m e c a lp e R tn e m h s ib ru fe R y g re n e la n o ita re p Oe s u re ta w la n o ita re p Oe s u n o itc u rts n o c -e Dn o itilo m e d tro p s n a rT g n is s e c o rp e ts a W la s o p s iD -e s u e R-y re v o c e R-g n ilc y c e Rla itn e to p
A1 A2 A3 A4 A5 B1 B2 B3 B4 B5 B6 B7 C1 C2 C3 C4 D
X X X X X MND MND MNR MNR MNR MND MND X X MND X X
RESULTS OF THE LCA - ENVIRONMENTAL IMPACT according to EN 15804+A2: 1 kg of Sika ViscoCrete®-2100
Parameter Unit A1-A3 A4 A5 C1 C2 C4 D
GWP-total kg CO 2 eq 1.26E+00 2.59E-01 2.64E-02 2.92E-04 6.48E-03 4.33E-02 -3E-03
GWP-fossil kg CO 2 eq 1.25E+00 2.48E-01 2.05E-02 2.8E-04 6.21E-03 4.29E-02 -2.99E-03
GWP-biogenic kg CO 2 eq 1.12E-02 1.06E-02 5.95E-03 1.2E-05 2.64E-04 4.41E-04 -1.32E-06
GWP-luluc kg CO 2 eq 1.52E-04 8.18E-06 1.72E-06 9.36E-09 2.04E-07 1.53E-05 -2.04E-07
ODP kg CFC11 eq 2.91E-12 2.32E-14 3.07E-14 2.65E-17 5.79E-16 6.67E-14 -1.06E-14
AP mol H+ eq 2.14E-03 6.51E-04 4.04E-05 3.57E-06 1.79E-05 2.12E-04 -4.18E-06
EP-freshwater kg P eq 7.17E-06 5.88E-08 7.27E-08 6.72E-11 1.47E-09 1.33E-07 -1.56E-09
EP-marine kg N eq 7.38E-04 3.2E-04 1.37E-05 1.65E-06 8.83E-06 5.73E-05 -9.25E-07
EP-terrestrial mol N eq 8.22E-03 3.51E-03 1.57E-04 1.8E-05 9.72E-05 6.3E-04 -9.99E-06
kg NMVOC
POCP 2.09E-03 6.22E-04 3.61E-05 4.92E-06 1.7E-05 1.57E-04 -2.65E-06
eq
ADPE kg Sb eq 5.92E-07 8.1E-08 6.17E-09 9.26E-11 2.02E-09 1.14E-08 -5.81E-10
ADPF MJ 3.13E+01 3.35E+00 3.67E-01 3.83E-03 8.36E-02 6.22E-01 -4.65E-02
m3 world eq
WDP 3.47E-01 1.43E-03 4.81E-03 1.64E-06 3.58E-05 2.6E-03 -5.84E-04
deprived
GWP = Global warming potential; ODP = Depletion potential of the stratospheric ozone layer; AP = Acidification potential of land and water; EP =
Eutrophication potential; POCP = Formation potential of tropospheric ozone photochemical oxidants; ADPE = Abiotic depletion potential for non-fossil
resources; ADPF = Abiotic depletion potential for fossil resources; WDP = Water (user) deprivation potential)
RESULTS OF THE LCA - INDICATORS TO DESCRIBE RESOURCE USE according to EN 15804+A2: 1 kg of Sika ViscoCrete®-
2100
Parameter Unit A1-A3 A4 A5 C1 C2 C4 D
PERE MJ 1.85E+00 2.63E-02 1.97E-02 3E-05 6.55E-04 6.01E-02 -9.36E-03
PERM MJ 0 0 0 0 0 0 0
PERT MJ 1.85E+00 2.63E-02 1.97E-02 3E-05 6.55E-04 6.01E-02 -9.36E-03
PENRE MJ 2.69E+01 3.59E+00 3.71E-01 4.11E-03 8.97E-02 6.41E-01 -4.65E-02
PENRM MJ 4.82E+00 0 0 0 0 0 0
PENRT MJ 3.17E+01 3.59E+00 3.71E-01 4.11E-03 8.97E-02 6.41E-01 -4.65E-02
SM kg 0 0 0 0 0 0 0
RSF MJ 0 0 0 0 0 0 0
NRSF MJ 0 0 0 0 0 0 0
FW m3 1.06E-02 5.85E-05 1.37E-04 6.69E-08 1.46E-06 9.2E-05 -1.78E-05
PERE = Use of renewable primary energy excluding renewable primary energy resources used as raw materials; PERM = Use of renewable primary
energy resources used as raw materials; PERT = Total use of renewable primary energy resources; PENRE = Use of non-renewable primary energy
excluding non-renewable primary energy resources used as raw materials; PENRM = Use of non-renewable primary energy resources used as raw
materials; PENRT = Total use of non-renewable primary energy resources; SM = Use of secondary material; RSF = Use of renewable secondary fuels;
NRSF = Use of non-renewable secondary fuels; FW = Use of net fresh water
RESULTS OF THE LCA – WASTE CATEGORIES AND OUTPUT FLOWS according to EN 15804+A2:
1 kg of Sika ViscoCrete®-2100
Parameter Unit A1-A3 A4 A5 C1 C2 C4 D
HWD kg 2.34E-09 1.19E-11 2.43E-11 1.36E-14 2.96E-13 2.4E-11 -1.95E-12
NHWD kg 2.36E-02 1.59E-04 2.06E-03 1.82E-07 3.97E-06 1E+00 -1.54E-05
RWD kg 5.2E-04 9.69E-06 5.48E-06 1.11E-08 2.42E-07 5.63E-06 -4.19E-06
CRU kg 0 0 0 0 0 0 0
MFR kg 0 0 0 0 0 0 0
MER kg 0 0 0 0 0 0 0
EEE MJ 0 0 1.93E-02 0 0 0 0
EET MJ 0 0 3.49E-03 0 0 0 0
4 Environmental Product Declaration - Sika - Sika ViscoCrete®-2100
HWD = Hazardous waste disposed; NHWD = Non-hazardous waste disposed; RWD = Radioactive waste disposed; CRU = Components for re-use;
MFR = Materials for recycling; MER = Materials for energy recovery; EEE = Exported electrical energy; EET = Exported thermal energy
RESULTS OF THE LCA – additional impact categories according to EN 15804+A2-optional:
1 kg of Sika ViscoCrete®-2100
Parameter Unit A1-A3 A4 A5 C1 C2 C4 D
Disease
PM ND ND ND ND ND ND ND
incidence
IR kBq U235 eq ND ND ND ND ND ND ND
ETP-fw CTUe ND ND ND ND ND ND ND
HTP-c CTUh ND ND ND ND ND ND ND
HTP-nc CTUh ND ND ND ND ND ND ND
SQP SQP ND ND ND ND ND ND ND
PM = Potential incidence of disease due to PM emissions; IR = Potential Human exposure efficiency relative to U235; ETP-fw = Potential comparative
Toxic Unit for ecosystems; HTP-c = Potential comparative Toxic Unit for humans (cancerogenic); HTP-nc = Potential comparative Toxic Unit for humans
(not cancerogenic); SQP = Potential soil quality index
Disclaimer 1 – for the indicator “Potential Human exposure efficiency relative to U235”. This impact category deals mainly with the
eventual impact of low-dose ionizing radiation on human health of the nuclear fuel cycle. It does not consider effects due to possible
nuclear accidents, occupational exposure or radioactive waste disposal in underground facilities. Potential ionizing radiation from the
soil, radon and from some construction materials is also not measured by this indicator.
Disclaimer 2 – for the indicators “abiotic depletion potential for non-fossil resources”, “abiotic depletion potential for fossil resources”,
“water (user) deprivation potential, deprivation-weighted water consumption”, “potential comparative toxic unit for ecosystems”,
“potential comparative toxic unit for humans – cancerogenic”, “Potential comparative toxic unit for humans - not cancerogenic”,
“potential soil quality index”. The results of this environmental impact indicator shall be used with care as the uncertainties on these
results are high as there is limited experience with the indicator.
This EPD was created using a software tool.
References
Code of Federal Regulations Title 29, Subtitle B, Chapter XVII,
AASHTO M194 Part 1910, Subpart Z, Section 1910.1200 Hazard
Standard Specification for Chemical Admixtures for Concrete communication.
ASTM C494/C494M
Standard Specification for Chemical Admixtures for Concrete Further References
ASTM E70 IBU 2021
Standard Test Method for pH of Aqueous Solutions With the Institut Bauen und Umwelt e.V.: General Instructions for the
Glass Electrode EPD programme of Institut Bauen und Umwelt e.V., Version
2.0, Berlin: Institut Bauen und Umwelt e.V., 2021 www.ibu-
Clean Air Act (CAA) epd.com
42 U.S.C. §7401 et seq. (1970)
LCA Calculator
EN 480-10 LCA Calculator software (version 6). Visualize, Improve and
Admixtures for concrete, mortar and grout. Test methods. Report on Product Sustainability. https://sphera.com/your-path-
Determination of water soluble chloride content to-sustainability/
EN 15804 LCA for Expert
EN 15804:2012+A1:2013, Sustainability of construction works Life cycle assessment software (version 10), by Sphera
— Environmental Product Declarations — Core rules for the Solutions GmbH, Leinfelden-Echterdingen, 2022
product category of construction products. https://sphera.com/life-cycle-assessment-lca-software/
EN 15804 Managed LCA Content
EN 15804:2012+A2:2019+AC:2021, Sustainability of Life cycle assessment database, by Sphera Solutions GmbH,
construction works — Environmental Product Declarations — Leinfelden-Echterdingen, 2022
Core rules for the product category of construction products. https://sphera.com/life-cycle-assessment-lca-database/
ISO 14025 PCR Part A
EN ISO 14025:2011, Environmental labels and declarations — PCR - Part A: Calculation rules for the Life Cycle Assessment
Type III environmental declarations — Principles and and Requirements on the Background Report, version 1.3,
procedures. Institut Bauen und Umwelt e.V., 08-2021.
OSHA 29CFR 1910.1003 PCR Part B
Code of Federal Regulations Title 29, Subtitle B, Chapter XVII, PCR – Part B:Requirements on the EPD for Concrete
Part 1910, Subpart Z, Section 1910.1003 13 Carcinogens. admixtures, Institut Bauen und Umwelt e.V., 04-2023.
OSHA 29CFR 1910.1200
5 Environmental Product Declaration - Sika - Sika ViscoCrete®-2100
Publisher
Institut Bauen und Umwelt e.V. +49 (0)30 3087748- 0
Hegelplatz 1 info@ibu-epd.com
10117 Berlin www.ibu-epd.com
Germany
Programme holder
Institut Bauen und Umwelt e.V. +49 (0)30 3087748- 0
Hegelplatz 1 info@ibu-epd.com
10117 Berlin www.ibu-epd.com
Germany
Author of the Life Cycle Assessment
Sphera Solutions GmbH +49 711 341817-0
Hauptstraße 111- 113 info@sphera.com
70771 Leinfelden-Echterdingen www.sphera.com
Germany
Owner of the Declaration
Sika Corporation +1-800-933-7452
Polito Avenue 201 product.sustainability@ch.sika.com
07071 Lyndhurst, NJ usa.sika.com/sustainability
United States
6 Environmental Product Declaration - Sika - Sika ViscoCrete®-2100
