ENVIRONMENTAL PRODUCT DECLARATION
as per ISO 14025 and EN 15804+A2
Owner of the Declaration IGI - The Global Wallcoverings Association
Publisher Institut Bauen und Umwelt e.V. (IBU)
Programme holder Institut Bauen und Umwelt e.V. (IBU)
Declaration number EPD-IGI-20230435-IBG1-EN
Issue date 18.01.2024
Valid to 17.01.2029
Wallcoverings on non-woven base
IGI - The Global Wallcoverings Association
www.ibu-epd.com | https://epd-online.com
1. General Information
IGI - The Global Wallcoverings Association Wallcoverings on non-woven base
Programme holder Owner of the declaration
IBU – Institut Bauen und Umwelt e.V. IGI - The Global Wallcoverings Association
Hegelplatz 1 Chaussée de Louvain 426
10117 Berlin 1380 LASNE
Germany Belgium
Declaration number Declared product / declared unit
EPD-IGI-20230435-IBG1-EN The declared unit is 1m² (square meter) decorative wallcovering on non-
woven base including packaging.
This declaration is based on the product category rules: Scope:
Wall coverings, 01.08.2021 This EPD focuses on the production, transport and disposal of a weighted
(PCR checked and approved by the SVR) average of 1m² wallcoverings on non-woven base of participating
members of the IGI - The Global Wallcoverings Association.
Non-decorative wallcoverings for a later additional treatment like painting
Issue date ("whites") are included in this scope as they follow a worst case approach.
16 out of 71 IGI members are involved in this EPD: A.S. Création Tapeten
18.01.2024
AG (DE), Anstey Wallpaper Co. Ltd (GB), BN International (NL), Borås
Tapetfabrik AB (SE), Decoprint NV (BE), Erfurt & Sohn KG (DE), Fine
Decor Wallcoverings Ltd (GB), Flügger A/S (DK), Grandeco NV (BE), JV
Valid to
S.p.A. (IT), Marburger Tapetenfabrik J.B. Schaefer GmbH & Co. KG (DE),
17.01.2029 Rasch GmbH & Co. KG (DE), Roysons Corporation (US), The Surface
Print Company Ltd (GB), UGÉPA SA (FR), York Wallcoverings inc. (US).
The technical properties are displayed in chapter 2.3.
The owner of the declaration shall be liable for the underlying information
and evidence; the IBU shall not be liable with respect to manufacturer
information, life cycle assessment data and evidences.
The EPD was created according to the specifications of EN 15804+A2. In
the following, the standard will be simplified as EN 15804.
Verification
The standard EN 15804 serves as the core PCR
Dipl.-Ing. Hans Peters
Independent verification of the declaration and data according to ISO
(Chairman of Institut Bauen und Umwelt e.V.)
14025:2011
internally X externally
Florian Pronold Prof. Dr. Birgit Grahl,
(Managing Director Institut Bauen und Umwelt e.V.) (Independent verifier)
1 Environmental Product Declaration - IGI - The Global Wallcoverings Association - Wallcoverings on non-woven base
2. Product
2.1 Product description/Product definition 1b
Wallcoverings on non-woven base according to EN 15102 Performance Category I, II, III, IV, V or VI as described in Table
involve a non-woven base. A non-woven base is a substrate 1 of F 793-0-06 should be declared.
composed of a blend of cellulose and polyester fibres. Non-
woven wallcovering is dimensionally stable to aqueous paste 2.4 Delivery status
and does not require a soak time. When the wallcovering is to The products declared are provided within the following
be changed it can be stripped in its entirety by peeling the dimensions:
wallcovering lengths from the wall.
This property as defined in EN 235 is strippable.
For the placing on the market of the product in the European
Union/European Free Trade Association (EU/EFTA) (with the
exception of Switzerland) Regulation (EU) No. 305/2011 (CPR)
applies. The product needs a Declaration of Performance
This table contains the range of all wallcoverings examined. For
taking into consideration EN 15102 and CE-marking. For the
more precise information please contact the specific
application and use the respective national provisions apply.
manufacturer.
For the placing on the market in Great Britain the product 2.5 Base materials/Ancillary materials
needs a Declaration of Performance taking into consideration
The weighted average of the primary product components is
BS EN 15102 and UK Conformity Assessed (UKCA) marking.
shown in the following table, in percentage:
Name ValueUnit
For placing on the market in Northern Ireland the product needs
a Declaration of Performance taking into consideration (BS) EN Carrier material (Non-Woven, 80% Paper 20%
71 %
15102 and CE or CE and UK Northern Ireland (UKNI) marking. PET)
Packaging 10 %
For the placing on the market in the USA the product should Additives 11 %
conform to ASTM F 1141 – 93 Standard Specification for
Ink & Pigment 8
Wallcovering and ASTM F 793 – 06 Standard Classification of
Sum 100 %
Wall Covering by Use Characteristics.
Pallets were considered as part of the packaging.
2.2 Application
Wallcoverings are used for the decorative wall design of interior This product contains substances listed in the candidate list
spaces in private or commercial use. (date: 06.12.2023) exceeding 0.1 percentage by mass: no.
This product contains other CMR substances in categories 1A
2.3 Technical Data
or 1B that are not on the candidate list, exceeding 0.1
In accordance with EN 233, the following technical (structural)
percentage by mass: yes, vinyl acetate CAS no.: 108-05-4.
data can be declared on delivery:
Biocide products were added to this construction product or it
Constructional data has been treated with biocide products (this then concerns a
treated product as defined by the (EU) Ordinance on Biocide
Name Value Unit
Products No. 528/2012): no
Measures by categories EN 233 category 1 - 3 -
Ancillary materials of the phthalate chemical group, specifically
Straightness and parallelism in mm.
equal or less than 1 - Diisononyl phthalate (DINP) and Dioctyl Terephthalate (DOTP),
according to EN 12956
remain on the product and serve the function of softeners.
spongeable to This EPD is a weighted average of a Manufacturer Group
Washability according to EN 12956 -
extra-washable regarding several producers and product references. Therefore,
Colour fastness to light according to it cannot be ruled out that individual wallcoverings may contain
3 - 6 -
EN ISO 105-B02 small amounts (>0.1% of product weight) of substances that
Migration of heavy metals and certain are included in the Substance of Very High Concern SVHC
other elements to EN 12149 fulfills the norm - candidate list, the CMR substances in categories 1A or 1B list
or ancillary materials and additives serving the function of fire
Emissions of formaldehyde max.
fulfills the norm - retardants, softeners or biocides.
< 120 mg/kg according to EN 12149
This can be attributed, for example, to the contents of used
In case of multiple answers, values need to be examined waste paper.
depending on the manufacturer. Further information can be obtained from the respective
For USA manufactured products should be in accordance with manufacturer.
ASTM F 793-0-06 Table 1 Classification Criteria.
Depending on whether products are intended for the European, 2.6 Manufacture
UK or US market, the following performance data must be The manufacturing process can be described with the help of
declared. the following graphic:
1a: Product according to the CPR, based on (BS) EN
15102:
Performance data of the product in accordance with the
Declaration of Performance with respect to its Essential
Characteristics according to EN 15102.
or:
2 Environmental Product Declaration - IGI - The Global Wallcoverings Association - Wallcoverings on non-woven base
Building Assessment System (BNB).
Description of the influences on the ageing of the product when
applied in accordance with the rules of technology.
2.13 Extraordinary effects
Fire
The reaction to fire performance according to /EN 13501/ is
shown in the following table:*
Fire protection
Name Value
Building material class B-D
Burning droplets s1-s3
Smoke gas development d0-d2
*This table contains the range of all wallcoverings examined.
The order of manufacture may change and can slightly deviate
For more precise information please contact the specific
for different producers.
manufacturer.
2.7 Environment and health during manufacturing
For USA information on fire performance according to ASTM E
Compliance with statutory health and safety for personnel is
84 Test method for Surface Burning Characteristics of Building
ensured. Further, the energy and environmental management
Materials.
is certified for some members according to ISO 14001 and ISO
50001.
For greater detail please contact the specific manufacturer.
Water
2.8 Product processing/Installation The product is not water resistant. There is no risk of a
Depending on the manufacturers suggestion, the adhesive is hazardous environmental impact in the event of water flooding.
applied to the back of the wallcovering or the substrate using a
wallpaper brush or short-napped roller. The wallcovering is Mechanical destruction
pressed against the wall and is cut along the top and bottom There is no risk of a hazardous environmental impact following
edge to fit the wall. unforeseen mechanical destruction.
2.9 Packaging 2.14 Re-use phase
Product is wrapped in clear shrink wrap, packed in corrugated The product is not re-usable.
cardboard boxes and palletised.
2.15 Disposal
2.10 Condition of use Wallcoverings are subject to the waste code 170904 (mixed
There are no special features to be noted within the limits of construction and demolition waste other than those mentioned
normal and customary usage. in 170901, 170902 and 170903) in accordance with the
European Waste Catalogue (EWC).
2.11 Environment and health during use Wallcoverings can therefore be disposed of as normal
No environmental problems can be expected when the product household waste, that is in the dustbin or in additional refuse
is handled and used sacks. Used wallcoverings should not be placed in the waste
properly. paper bank. Most household waste is incinerated or landfilled
depending on regional legal regulations in the EU or in the US.
2.12 Reference service life
Given the wallcovering is professionally installed, the reference 2.16 Further information
service life is 10 years according to the German Sustainable For further information please visit www.igiwallcoverings.org.
3. LCA: Calculation rules
3.1 Declared Unit 3.2 System boundary
The declared unit is 1 m² of wallcovering including packaging. Type of the EPD: cradle to gate - with options. The EPD is
The model is based on a weighted average of the produced considered a declaration of an average product as calculated
square meters of each participating manufacturer. from the output of several manufacturers (2b).
Declared unit
Module A1-3, A4 and A5
Name Value Unit
The product stage begins with the consideration of the
Declared unit 1 m2 production of the necessary raw materials and energies
Grammage 0.178 kg/m2 including all corresponding upstream processes as well as
transport.
Conversion factor to 1 kg 5.631 -
Furthermore, the entire production phase was investigated,
Layer thickness 0.001 m
including the treatment of production waste until reaching the
Density 1776 kg/m3 end-of-waste status (EoW). In addition, distribution transport
and installation in the building were taken into account.
The production processes and location may vary between
individual companies. The weighted average represents the
Modules C1-4
most likely scenario by production volumes and the selected
The modules include the environmental impacts of the removal
datasets correspond to all regarded regions.
and waste treatment until reaching the end-of-waste status
3 Environmental Product Declaration - IGI - The Global Wallcoverings Association - Wallcoverings on non-woven base
(EoW) including the associated transport at the end of the the basis of evaluations of the internal production and
product life cycle. environmental data, the collection of LCA-relevant data within
the supply chain as well as through the measurement of
Modules D relevant energy supply data. The collected data were checked
Calculation of potential benefits through the generated energy for plausibility and consistency. A good representation is to be
(electric & thermic) by the incineration processes in the life assumed.
cycle stages in A5 C3 and C4. The burdens resulting from the The data were collected in 2022 and refer to the calendar year
waste-to-energy plants are assigned in module C3 or C4 in 2021.
case of landfill gas combustion.
3.7 Period under review
3.3 Estimates and assumptions The LCA data were collected for the calendar year 2021.
'Non-woven' lacks information on the proportions of cellulose
and polyester. According to one manufacturer it contains 80% 3.8 Geographic Representativeness
cellulose and 20% polyester (PET). These proportions were Land or region, in which the declared product system is
applied to all other non-woven carrier materials. manufactured, used or handled at the end of the product´s
Most solvents were modelled as a generic mix of solvents. lifespan: Global
3.4 Cut-off criteria
3.9 Allocation
No materials were cut-off from the study. No energy
consumption was neglected. Potential benefits resulting from the thermal utilization of the
packaging waste (module A5) as well as from the thermal
3.5 Background data utilization or landfilling of the wallcoverings at the end of life
For modeling the lifecycle, the LCA for Experts Software (modules C3 and C4) are allocated to module D.
System and Database for Life Cycle Engineering (GaBi)
3.10 Comparability
Service pack 2023.1 was used. All background data records
relevant for production and disposal were almost exclusively Basically, a comparison or an evaluation of EPD data is only
taken from various GaBi supplementary databases or rarely possible if all the data sets to be compared were created
also from ecoinvent (v.3.6). The data records included in the according to EN 15804 and the building context, respectively
databases are documented online. the product-specific characteristics of performance, are taken
into account. The used background database is GaBi service
3.6 Data quality package 1 of 2023.
Data collection for the investigated products was carried out on
4. LCA: Scenarios and additional technical information
Installation into the building (A5)
Characteristic product properties of biogenic carbon
The treatment of packaging as waste was modeled in Module
The biogenic carbon content quantifies the amount of biogenic
A5 as a weighted average. The following table depicts the
carbon in a construction product leaving the factory gate, and it
packaging materials treated in A5 with more than 1 gram of
is separately declared for the product and for any
participation in the weighted average.
accompanying packaging.
Modules B1-B7 are deemed not relevant since the product
Information on describing the biogenic Carbon Content at needs no maintenance or operational energy or water use and
factory gate are, therefore, not declared.
Name ValueUnit Name Value Unit
Biogenic carbon content in product 0.036 kg Cardboard 0.009 kg
C
Pallet 0.009 kg
Biogenic carbon content in accompanying kg
0.004 Paper 0.001 kg
packaging C
Polyethylene 0.001 kg
Note: 1 kg of biogenic carbon is equivalent to 44/12 kg of CO .
2
Reference service life
Name Value Unit
Reference service life 10 a
Transport to the building site (A4)
End of life (C1-C4)
Name Value Unit
Name Value Unit
Capacity utilisation (including empty runs) 80 - 90 %
Incineration 98 %
Truck transport 27 t payload
Landfill 2 %
Transport distance 389 km
Train transport 726 t payload For the calculation of this LCA landfilling is chosen for the US
and incineration for the EU. Different disposal routes are
Transport distance 15 km
available but not taken into account for this industry average
Ship transport 27500 dwt payload
LCA.
Transport distance 174 km
Cargo plane transport 65 t payload Reuse, recovery and/or recycling potentials (D), relevant
Transport distance 29 km scenario information
In module D the potential benefits of the thermal combustion of
Because many different countries are involved, there were
the wallcoverings (C3) and their packaging (A5) as well as the
always global data sets used to model the transport distances.
incineration of landfill gases (C4) are displayed.
4 Environmental Product Declaration - IGI - The Global Wallcoverings Association - Wallcoverings on non-woven base
The benefits from thermal combustion of the wallcoverings are 73,3% of recycled paper in product does not receive benefits,
calculated in Module D. From the total paper used as backing, as it is a secondary material coming burden-free to the system.
5 Environmental Product Declaration - IGI - The Global Wallcoverings Association - Wallcoverings on non-woven base
5. LCA: Results
In this section, the LCA results for 1 m² wallcoverings are presented. It should be borne in mind that the LCA results only indicate
possible effects.
Indicators used for evaluation:
The EN 15804+A2 LCIA methodology with the characterization factors infrom EU-JRC were used to evaluate the possible
environmental effects of the wallcoverings. The characterization factors are available at the following internet link:
http://eplca.jrc.ec.europa.eu/LCDN/developerEF.xhtml.
DESCRIPTION OF THE SYSTEM BOUNDARY (X = INCLUDED IN LCA; MND = MODULE OR INDICATOR NOT DECLARED; MNR
= MODULE NOT RELEVANT)
Benefits and
Construction loads beyond
Product stage Use stage End of life stage
process stage the system
boundaries
la ire ta m w a Ry lp p u s tro p s n a rT g n iru tc a fu n a M e h t m o rf tro p s n a rTe tis e h t o t e ta g y lb m e s s A e s U e c n a n e tn ia M ria p e R tn e m e c a lp e R tn e m h s ib ru fe R y g re n e la n o ita re p Oe s u re ta w la n o ita re p Oe s u n o itc u rts n o c -e Dn o itilo m e d tro p s n a rT g n is s e c o rp e ts a W la s o p s iD -e s u e R-y re v o c e R-g n ilc y c e Rla itn e to p
A1 A2 A3 A4 A5 B1 B2 B3 B4 B5 B6 B7 C1 C2 C3 C4 D
X X X X X MND MND MNR MNR MNR MND MND X X X X X
RESULTS OF THE LCA - ENVIRONMENTAL IMPACT according to EN 15804+A2: 1 m² wallcoverings on non-woven base
Parameter Unit A1-A3 A4 A5 C1 C2 C3 C4 D
GWP-total kg CO 2 eq 1.79E-01 3.41E-02 1.75E-02 2.66E-05 1.48E-03 2.3E-01 1.97E-03 -8.04E-02
GWP-fossil kg CO 2 eq 3.27E-01 3.4E-02 4.09E-03 2.66E-05 1.47E-03 9.92E-02 2.13E-04 -8.04E-02
GWP-biogenic kg CO 2 eq -1.45E-01 0 1.34E-02 0 0 1.3E-01 1.76E-03 0
GWP-luluc kg CO 2 eq -2.87E-03 5.71E-05 1.09E-06 8.89E-09 1.36E-05 3.17E-06 1.42E-07 -5.08E-06
ODP kg CFC11 eq 7.73E-10 2.73E-15 1.86E-15 1.62E-16 1.91E-16 4.73E-14 2.81E-16 -5.99E-13
AP mol H+ eq 1.02E-03 1.65E-04 4.98E-06 6.73E-08 1.23E-05 6.05E-05 7.69E-07 -9.73E-05
EP-freshwater kg P eq 2.77E-05 2.7E-08 8.71E-09 2.34E-09 5.36E-09 1.63E-08 3.16E-08 -1.24E-07
EP-marine kg N eq 3.55E-04 7.41E-05 1.94E-06 2.36E-08 6.11E-06 2.08E-05 4.57E-07 -2.87E-05
EP-terrestrial mol N eq 3.52E-03 8.13E-04 2.31E-05 1.63E-07 6.75E-05 2.75E-04 2.65E-06 -3.08E-04
kg NMVOC
POCP 8.77E-04 1.93E-04 5.02E-06 4.41E-08 1.16E-05 5.51E-05 1.45E-06 -8.01E-05
eq
ADPE kg Sb eq 6.26E-08 6.82E-10 2.44E-11 1.53E-12 9.65E-11 4.16E-10 4.47E-12 -5.52E-09
ADPF MJ 6.58E+00 4.58E-01 6.84E-03 4.75E-04 2E-02 1.04E-01 2.5E-03 -1.46E+00
m3 world eq
WDP 3.09E-01 1.18E-04 1.93E-03 8.59E-03 1.77E-05 2.77E-02 8.06E-06 -7.26E-03
deprived
GWP = Global warming potential; ODP = Depletion potential of the stratospheric ozone layer; AP = Acidification potential of land and water; EP =
Eutrophication potential; POCP = Formation potential of tropospheric ozone photochemical oxidants; ADPE = Abiotic depletion potential for non-fossil
resources; ADPF = Abiotic depletion potential for fossil resources; WDP = Water (user) deprivation potential)
RESULTS OF THE LCA - INDICATORS TO DESCRIBE RESOURCE USE according to EN 15804+A2: 1 m² wallcoverings on non-
woven base
Parameter Unit A1-A3 A4 A5 C1 C2 C3 C4 D
PERE MJ 1.82E+00 7.58E-03 2.72E-01 9.67E-05 1.45E-03 2.1E+00 2.17E-02 -4.09E-01
PERM MJ 2.36E+00 0 -2.71E-01 0 0 -2.07E+00 -2.15E-02 0
PERT MJ 4.18E+00 7.58E-03 1.27E-03 9.67E-05 1.45E-03 2.74E-02 2.26E-04 -4.09E-01
PENRE MJ 5.48E+00 4.6E-01 6.13E-02 4.75E-04 2E-02 1.13E+00 3.31E-02 -1.46E+00
PENRM MJ 1.11E+00 0 -5.45E-02 0 0 -1.02E+00 -3.06E-02 0
PENRT MJ 6.59E+00 4.6E-01 6.85E-03 4.75E-04 2E-02 1.04E-01 2.5E-03 -1.46E+00
SM kg 9.18E-03 0 0 0 0 0 0 0
RSF MJ 0 0 0 0 0 0 0 0
NRSF MJ 0 0 0 0 0 0 0 0
FW m3 7.49E-03 8.6E-06 4.54E-05 2E-04 1.59E-06 6.57E-04 2.68E-07 -3.32E-04
PERE = Use of renewable primary energy excluding renewable primary energy resources used as raw materials; PERM = Use of renewable primary
energy resources used as raw materials; PERT = Total use of renewable primary energy resources; PENRE = Use of non-renewable primary energy
excluding non-renewable primary energy resources used as raw materials; PENRM = Use of non-renewable primary energy resources used as raw
materials; PENRT = Total use of non-renewable primary energy resources; SM = Use of secondary material; RSF = Use of renewable secondary fuels;
NRSF = Use of non-renewable secondary fuels; FW = Use of net fresh water
RESULTS OF THE LCA – WASTE CATEGORIES AND OUTPUT FLOWS according to EN 15804+A2:
1 m² wallcoverings on non-woven base
Parameter Unit A1-A3 A4 A5 C1 C2 C3 C4 D
HWD kg 3.33E-06 9.51E-13 2.21E-13 1.35E-14 6.21E-14 1.99E-12 2.1E-13 -8.46E-11
NHWD kg 2.02E-02 4.68E-05 1.13E-03 6.08E-05 3.06E-06 1.74E-02 2.12E-03 -7.09E-04
RWD kg 1.08E-04 5.68E-07 2.54E-07 1.9E-08 3.75E-08 5.02E-06 2.96E-08 -1.09E-04
6 Environmental Product Declaration - IGI - The Global Wallcoverings Association - Wallcoverings on non-woven base
CRU kg 0 0 0 0 0 0 0 0
MFR kg 0 0 0 0 0 0 0 0
MER kg 1.73E-02 0 1.02E-02 0 0 1.45E-01 0 0
EEE MJ 3.71E-02 0 0 0 0 0 0 3.61E-01
EET MJ 7.01E-02 0 0 0 0 0 0 7.01E-01
HWD = Hazardous waste disposed; NHWD = Non-hazardous waste disposed; RWD = Radioactive waste disposed; CRU = Components for re-use;
MFR = Materials for recycling; MER = Materials for energy recovery; EEE = Exported electrical energy; EET = Exported thermal energy
RESULTS OF THE LCA – additional impact categories according to EN 15804+A2-optional:
1 m² wallcoverings on non-woven base
Parameter Unit A1-A3 A4 A5 C1 C2 C3 C4 D
Disease
PM 8.53E-09 7.01E-10 3.05E-11 1.08E-12 8.72E-11 4.37E-10 7.46E-12 -8.26E-10
incidence
IR kBq U235 eq 7.95E-02 8.15E-05 4.02E-05 2.91E-06 5.59E-06 7.51E-04 4.37E-06 -1.81E-02
ETP-fw CTUe 9.36E+00 3.22E-01 4.01E-03 9.77E-04 1.42E-02 4.97E-02 2.59E-03 -3.08E-01
HTP-c CTUh 7.92E-10 6.04E-12 1.97E-13 1.86E-14 2.92E-13 2.74E-12 1.12E-13 -1.6E-11
HTP-nc CTUh 7.64E-08 3.34E-10 1.2E-11 1.74E-12 1.77E-11 1.61E-10 1.2E-11 -5.02E-10
SQP SQP 8.81E+00 3.6E-02 1.98E-03 7.06E-05 8.34E-03 2.88E-02 2.2E-04 -2.69E-01
PM = Potential incidence of disease due to PM emissions; IR = Potential Human exposure efficiency relative to U235; ETP-fw = Potential comparative
Toxic Unit for ecosystems; HTP-c = Potential comparative Toxic Unit for humans (cancerogenic); HTP-nc = Potential comparative Toxic Unit for humans
(not cancerogenic); SQP = Potential soil quality index
Disclaimer 1 – for the indicator “Potential Human exposure efficiency relative to U235”. This impact category deals mainly with the
eventual impact of low-dose ionizing radiation on human health of the nuclear fuel cycle. It does not consider effects due to possible
nuclear accidents, occupational exposure or radioactive waste disposal in underground facilities. Potential ionizing radiation from the
soil, radon and from some construction materials is also not measured by this indicator.
Disclaimer 2 – for the indicators “abiotic depletion potential for non-fossil resources”, “abiotic depletion potential for fossil resources”,
“water (user) deprivation potential, deprivation-weighted water consumption”, “potential comparative toxic unit for ecosystems”,
“potential comparative toxic unit for humans – cancerogenic”, “Potential comparative toxic unit for humans - not cancerogenic”,
“potential soil quality index”. The results of this environmental impact indicator shall be used with care as the uncertainties on these
results are high as there is limited experience with the indicator.
This EPD was created using a software tool.
6. LCA: Interpretation
7 Environmental Product Declaration - IGI - The Global Wallcoverings Association - Wallcoverings on non-woven base
incineration in a waste-to-energy facility, it is treated as a load
The production stage (module A1-A3) clearly dominates the (C3). Moreover, paper production has the highest influence on
LCA results. The loads caused by the disposal stage (modules the acidification potential (AP), the eutrophication potential
C3 and C4) become noticeable, especially as the biogenic (EP), the ozone depletion (ODP), and the Potential for the
carbon leaves the product system, reflected in the total and formation of tropospheric ozone (POCP).
biogenic global warming potential. Transports play a Transport processes also affect GWP-fossil, AP, EP POCP, and
subordinate yet not insignificant role. ADPF. The main reason is the combustion of fuels.
The main environmental impacts are in all categories located in
module A1-A3. For GWP-fossil and ADPF the highest precursor Range of the results
of impact is the production of non-woven backing, made up of The individual results of the participating companies differ from
paper and PET fibers. The generation of thermal energy for the average results in the present environmental product
general production and heating/drying processes in A3 is the declaration. Regarding GWP, the results may be 249% higher
second highest source of impact in the GWP-fossil category or 53% lower than the average for this EPD.
and ADPF; with the electricity use in third place. The main reason for the deviations is differences in the
The production of paper dominates most impact categories, as grammage of the individual wallcoverings. In addition, there are
it has a relatively high share of the greenhouse potential due to different materials used as well as varying heat and electricity
energy demands. In the GWP category, the biogenic carbon consumptions depending on the Manufacturer.
dioxide contained in the paper is treated first as a credit; after
7. Requisite evidence
Members of the The Global Wallcoverings Association have the wallcoverings meet the requirements of test standard
following certificates: ISO 16000.
• Optional compliance with German RAL-GZ 479.
• The declared products comply with EN 15102.
• Optional compliance with USA Wallcovering Association
• According to the (emission) test chamber assessment,
W-101 (2013) paragraph 8.1 when tested by California
which follows the French measurement method Arrêté
Specification Section 01350 to criteria CDPH/EHLB
du 19/04/11 the wallcoverings meet the requirements of
Standard Method V1.1 (2010).
the test standard ISO 16000.
The certificates and classifications for the various wallcoverings
• Optional according to the chamber test which follows
can be obtained from the respective manufacturers.
the German AgBB (Committee for health-related
evaluation of building products) regulations the
8. References
Standards and Norms and of formaldehyde release.
EN 12149:1997
Arrêté du 19/04/11 Wallcoverings in roll form - Determination of migration of heavy
Order of 19 April 2011 relating to the labeling of construction metals and certain other elements, of vinyl chloride monomer
products or wall or floor coverings and paints and varnishes on and of formaldehyde release.
their emissions of volatile pollutants
EN 12956:1999
ASTM E 84 Wallcoverings in roll form - Determination of dimensions,
ASTM E 84:2016: Standard Test Method for Surface Burning straightness, spongeability and washability.
Characteristics of Building Materials
EN 13501-1:2018
ASTM F 793 Fire classification of construction products and building
ASTM F793 / F793M-15, Standard Classification of Wall elements - Part 1: Classification using data from reaction to fire
Coverings by Use Characteristics, ASTM International, West Tests.
Conshohocken, PA, 2015
EN 15102:2007+A1:2011
ASTM F1141 - 93 Decorative wall coverings - Roll and panel form.
ASTM F1141-93(2009), Standard Specification for
Wallcovering, ASTM International, West Conshohocken, PA, EN 233:2016
2009 Wallcoverings in roll form - Specification for finished wallpapers,
wall vinyls and plastics wallcoverings.
BNB
Lifetimes of components for life cycle analyses according to the EN 234:2019
Bewertungssystem Nachhaltiges Bauen, 2011. Wallcoverings in roll form – Specification for wallcoverings for
subsequent decoration
CDPH/EHLB
Standard method for measuring and evaluating chemical EN 235:2001
emissions from indoor sources using environmental chambers, Wall coverings - Vocabulary and Symbols.
Version 1.1
EN 259-1:2001
CPR Wall coverings in roll form - Heavy duty wallcoverings - Part 1:
Construction Product Regulation EU Specifications.
EN 12149:1997
Wallcoverings in roll form - Determination of migration of heavy EN ISO 105-B02
metals and certain other elements, of vinyl chloride monomer Textiles - Tests for colour fastness - Part B02: Colour fastness
8 Environmental Product Declaration - IGI - The Global Wallcoverings Association - Wallcoverings on non-woven base
to artificial light: Xenon arc fading lamp test (ISO 105- construction products and repealing Council Directive
B02:2014). 89/106/EEC Text with EEA relevance. Current consolidated
version: 16/07/2021
EN ISO 14025:2006
Environmental labels and declarations — Type III WA-101
environmental declarations — Principles and procedures; 2009- WA Quality Standard for Polymer Coated Fabric Wallcovering
11.
EN ISO 14044:2006 Further documentation
Environmental management - Life cycle assessment -
Requirements and guidelines (ISO 14044:2006). Ecoinvent
Database for Life Cycle Assessment, version 3.6. Swiss Center
EN ISO 16000:2006 for Life Cycle Inventories, St. Gallen, 2023.
Indoor air - Part 3: Determination of formaldehyde and other
carbonyl compounds in indoor air and test chamber air - Active European Commission
sampling method. List of substances banned for use in cosmetic products. CMR
Indoor air - Part 6: Determination of volatile organic compounds substances of category 1A, 1B or 2 under Commission
in indoor and test chamber air by active sampling on Tenax Regulation (EC) No 790/2009. 01/12/2010. Updated
TA® sorbent, thermal desorption and gas chromatography 01/07/2015.
using MS or MS-FID.
Indoor air - Part 9: Determination of the emission of volatile European Parliament
organic compounds from building products and furnishing - Regulation (EU) no 528/2012 of the European Parliament and
Emission test chamber method. of the council of 22 may 2012 concerning the making available
Indoor air - Part 11: Determination of the emission of volatile on the market and use of biocidal products.
organic compounds from building products and furnishing -
Sampling, storage of samples and preparation of test European Waste Catalogue (EWC)
specimens. European Waste Catalogue / Ordinance on European List of
Wastes
ISO 14001:2015
Environmental management systems - Requirements with EU-JRC
guidance for use. EN 15804 reference package. Flows, Methods,
Characterisation Factors, Unit Groups and Flow Properties
EN 15804 based on EF Reference Package 3.0.
EN 15804:2012+A2:2019+AC:2021, Sustainability of
construction works — Environmental Product Declarations — German AgBB
Core rules for the product category of construction products. Committee for health-related evaluation of building products.
Umweltbundesamt Deutschlands.
ISO 50001:2011
Energy management systems - Requirements with guidance for Institut Bauen und Umwelt e. V.
use. Product Category Rules for Building-Related Products and
Services – PCR-A: Part A+A2: Calculation Rules for the Life
SVHC Cycle Assessment and Requirements on the Project Report
Candidate List of substances of very high concern for according to EN 15804+A2:2019, version: 1.3 from 31/08/2022.
Authorisation (SVHC)
Published in accordance with Article 59(10) of the REACH Institut Bauen und Umwelt e. V.
Regulation. European chemicals agency (ECHA). PCR Guidance-Texts for Building-Related Products and
Services - Part B: Requirements on the EPD for Wallcoverings.
RAL-GZ 479 Version: 8 from 01/08/2021.
Wallpapers - Quality assurance
LCA for Experts (GaBi)
Regulation (EU) No 305/2011 LCA for Experts 10.7.0.183: Software System and Database for
of the European Parliament and of the Council of 9 March 2011 Life Cycle Engineering. 1992-2023. Sphera Solutions GmbH
laying down harmonised conditions for the marketing of
9 Environmental Product Declaration - IGI - The Global Wallcoverings Association - Wallcoverings on non-woven base
Publisher
Institut Bauen und Umwelt e.V. +49 (0)30 3087748- 0
Hegelplatz 1 info@ibu-epd.com
10117 Berlin www.ibu-epd.com
Germany
Programme holder
Institut Bauen und Umwelt e.V. +49 (0)30 3087748- 0
Hegelplatz 1 info@ibu-epd.com
10117 Berlin www.ibu-epd.com
Germany
Author of the Life Cycle Assessment
brands & values GmbH +49 421 70 90 84 33
Altenwall 14 info@brandsandvalues.com
28195 Bremen www.brandsandvalues.com
Germany
Owner of the Declaration
IGI - The Global Wallcoverings Association +32 (0) 2 720 00 09
Chaussée de Louvain 426 info@igiwallcoverings.org
1380 LASNE www.igiwallcoverings.org
Belgium
10 Environmental Product Declaration - IGI - The Global Wallcoverings Association - Wallcoverings on non-woven base
