ENVIRONMENTAL PRODUCT DECLARATION
as per ISO 14025 and EN 15804+A2
Owner of the Declaration JANSEN AG
Publisher Institut Bauen und Umwelt e.V. (IBU)
Programme holder Institut Bauen und Umwelt e.V. (IBU)
Declaration number EPD-JAN-20230539-CBA1-EN
Issue date 16/07/2024
Valid to 15/07/2029
Janisol window width x height: 1230mm x 1480mm
Jansen AG
www.ibu-epd.com | https://epd-online.com
General Information
Jansen AG Janisol window width x height: 1230mm x 1480mm
Programme holder Owner of the declaration
IBU – Institut Bauen und Umwelt e.V. JANSEN AG
Hegelplatz 1 Industriestrasse 34
10117 Berlin 9463 Oberriet
Germany Switzerland
Declaration number Declared product / declared unit
EPD-JAN-20230539-CBA1-EN 1 m2 Janisol window with a grammage of 44.39 kg/m². The actual
reference size of the declared window has dimensions of width x height:
1230 mm x 1480 mm.
This declaration is based on the product category rules: Scope:
Windows and doors , 01/08/2021 The environmental product declaration refers to a window type Janisol in
(PCR checked and approved by the SVR) specific dimension width x height. The characteristic values used for the
system components Janisol in the LCA are provided by Jansen AG.
Issue date The declared product is defined according to the profile series and product
characteristics.
16/07/2024
The location of the production site is Oberriet/ Switzerland.
This EPD was created with the help of a semi-automatic LCA-Tool.
Valid to
The owner of the declaration shall be liable for the underlying information
15/07/2029 and evidence; the IBU shall not be liable with respect to manufacturer
information, life cycle assessment data and evidences.
The EPD was created according to the specifications of EN 15804+A2. In
the following, the standard will be simplified as EN 15804.
Verification
The standard EN 15804 serves as the core PCR
Independent verification of the declaration and data according to ISO
14025:2011
internally X externally
Dipl.-Ing. Hans Peters
(Chairman of Institut Bauen und Umwelt e.V.)
Florian Pronold Matthias Schulz,
(Managing Director Institut Bauen und Umwelt e.V.) (Independent verifier)
1 Environmental Product Declaration - Jansen AG - Janisol window width x height: 1230mm x 1480mm
Product
Constructional data
Product description/Product definition
Janisol windows are made of steel or stainless steel profiles Name Value Unit
with a depth of 60mm and a slender face width. This Resistance to wind load acc. to EN
C4 class
declaration describes the following element in Janisol: 12210
Product: Janisol Water tightness acc. to EN 12208 9A class
Width x height: 1230mm x 1480mm
Sound insulation class acc. to EN up to Rw 45 dB
Face width sash: 82.5mm / transom 103mm -
ISO 10140 (-2; -5)
Basic depth: 60mm / sash depth: 64mm
Heat transfer coefficient acc. to DIN
CE marking according to EN 14351-1 1.5 W/(m2K)
EN ISO 10077-2
The products require a declaration of performance taking into Air permeability acc. to EN 12207 4 class
account the harmonized product standard EN 14351-1 windows Mechanical strength acc. to EN
1 class
and doors and a CE marking. The respective national 13115
regulations apply to the use. With this declaration the following Bullet proofing acc. to EN 1522 FB4-FB6 class
element is declared: Burglar resistance acc. to EN 1627 RC1-RC3 class
Product according to the CPR, based on EN: Performance data
of the product in accordance with the declaration of
performance with respect to its essential characteristics
according to EN 14351-1, windows. Other constructional data
are not relevant for this product.
Base materials/Ancillary materials
JANSEN Janisol window is made of the following materials:
• Glazing approx. 34%
• Steel approx. 52%
• Plastics and fillers approx. 8%
• Fittings approx. 4%
• Aluminium 2%
The percentages relate to the most frequently sold product with
an opening of 1.82 m2. The percentages stated may vary
depending on the product type and dimensions.
Does the product or at least one part product contain materials
from the ECHA candidate list of materials which are especially
problematic for approval: Substances of Very High Concern –
SVHC (date 23.01.2024) above a mass % of 0.1: no.
This product/article/at least one partial article contains other
CMR substances in categories 1A or 1B which are not on the
candidate list, exceeding 0.1 percentage by mass: no.
Biocide products were added to this construction product or it
has been treated with biocide products (this then concerns a
treated product as defined by the (EU) Ordinance on Biocide
Products No. 528/2012): no.
Application
Reference service life
The Janisol opening element can be integrated for building
According to SBR 2011 regarding the specific material
ventilation and light transmission.
characteristics of steel windows and doors, the reference
service life is 75 years (SBR 2011). The practical service life
Technical Data
may well be longer. Conditions for a long service life are regular
According to the CE marking, the following structural data for
maintenance, care and upkeep of the product. The specified
the element must be stated:
service life is independent of the manufacturer's warranty.
LCA: Calculation rules
Name Value Unit
Declared Unit
Grammage 44.39 kg/m2
The declared unit is a 1 m2 of Janisol window element.
Declared unit 1 m2
The actual reference size of the declared window element has Layer thickness 0.06 m
dimensions of 1230 mm x 1480 mm.
For inhomogeneous components made of different materials,
Declared unit the conversion to other dimensions with factors leads to
deviations compared to the exact calculation. The frame
2 Environmental Product Declaration - Jansen AG - Janisol window width x height: 1230mm x 1480mm
percentage is 28.84% and the ground reference is 0.074 m². materials without heating value (except metals) including
glazing (C4/1).
frame percentage = frame surface / total area x 100 [%] Scenario 2 (module C3/2): 100% recycling of plastic system
ground reference = element depth x element width [m²] parts and 100% recycling of metal system components. Landfill
of all materials without heating value (except metals) including
System boundary glazing (C4/2).
Type of EPD according to EN 15804: "cradle to gate with Modules C4/1 & C4/2 are identical.
options, modules C1–C4, and module D". The following
modules are declared: A1–A3, C, D and additional modules: A4 EoL scenario 1 (modules C3/1 and C4/1)
+ A5. Collected separately waste type (window element) 44.39 kg
Recycling (C3/1) 25.54 kg
Production (modules A1-A3): Energy recovery (C3/1) 3.75 kg
Landfilling (C4/1) 15.26 kg
This module considers the provision of all relevant window
components (i.e. metal profiles/ components, glass units and EoL scenario 2 (modules C3/2 and C4/2)
plastic parts/profiles) and raw materials including their transport Collected separately (window element) 44.39 kg
to the declared production plant. This considers the Recycling (C3/2) 29.10 kg
manufacturing and assembly of these components, including Energy recovery (C3/2) 0.19 kg
waste processing up to the end-of-waste state. The impact of Landfilling (C4/2) 15.26 kg
packaging materials is also covered by this module.
Transport to the construction site (module A4): Benefits and loads beyond the product system boundary
(module D):
A distance of 100 km is considered for the transport of the
packed finished product via truck. The transport distance can Considers credits and loads from the recycling of the metal
be modified project-specific if required by linear scaling. components (duplicated in D/1 and D/2) and the recycling of
the plastic system parts/profiles (D/2). Avoided burdens from
Installation (module A5): the thermal treatment of all raw materials with heating value
(including plastic system parts/ profiles) (D/1) and packaging
Treatment and disposal of packaging material is considered in treatment (duplicated in D/1 and D/2) under European
this module. Credits for potential avoided burdens due to conditions are considered. This affects only the rate of primary
energy substitution of electricity and thermal energy generation materials (no secondary materials).
are declared in module D under European conditions and
affects only the rate of primary materials (no secondary Geographic Representativeness
materials). Land or region, in which the declared product system is
manufactured, used or handled at the end of the product´s
EoL stage (modules C1-C4): lifespan: Europe
Module C1 - considers manual deconstruction (without
Comparability
environmental burdens).
Module C2 - considers 50 km truck transport to waste Basically, a comparison or an evaluation of EPD data is only
processing. The transport distance can be modified project- possible if all the data sets to be compared were created
specific if required by linear scaling. according to EN 15804 and the building context, respectively
Modules C3 and C4 - consider waste processing and/or the product-specific characteristics of performance, are taken
disposal with the following scenarios: into account. The following background database has been
Scenario 1: 100% thermal treatment of all raw materials with used for the LCA calculation: Sphera LCA software (GaBi ts)
heating value including plastic system parts and 100% content update package (CUP) version 2022.2
recycling of metal system components (C3/1). Landfill of all
LCA: Scenarios and additional technical information
Janisol window.
Characteristic product properties of biogenic carbon
Transport to the building site (A4)
No biogenic carbon is reported in the product. The biogenic
carbon content in the accompanying packaging for 1 m2 Janisol Name Value Unit
window is declared below. Litres of fuel 0.0874 l/100km
Transport distance 100 km
Information on describing the biogenic Carbon Content at
factory gate Capacity utilisation (including empty runs) 61 %
Name Value Unit Gross weight of packed products transported 44.41 kg
kg
Biogenic carbon content in product - Installation into the building (A5)
C
Name Value Unit
Biogenic carbon content in accompanying kg
0.01318 Polyethylene (waste packaging to incineration) 0.00284 kg
packaging C
Cardboard box (waste packaging to incineration) 0.01360 kg
Note: 1kg of biogenic carbon is equivalent to 44/12 kg of CO2.
Wood (waste packaging to incineration) 0.01794 kg
According to SBR 2011 regarding the specific material
The following technical information is a basis for the declared characteristics of steel windows and doors, the reference
modules. The values refer to the declared unit of 1 m2 of service life is 75 years (SBR 2011). The practical service life
3 Environmental Product Declaration - Jansen AG - Janisol window width x height: 1230mm x 1480mm
may well be longer. Conditions for a long service life are regular plastics such as those present in the declared product.
maintenance, care and upkeep of the product. The specified Name Value Unit
service life is independent of the manufacturer's warranty.
EoL scenario 1 (modules C3/1 and C4/1)
Recycling (C3/1) 25.54 kg
Energy recovery (C3/1) 3.75 kg
Reference service life
Landfilling (C4/1) 15.26 kg
EoL scenario 2 (modules C3/2 and C4/2)
Name Value Unit
Recycling (C3/2) 29.10 kg
Life Span (according to SBR 2011) 75 a
Energy recovery (C3/2) 0.19 kg
Reference service life according to SBR 2011.
Landfilling (C4/2) 15.26 kg
Reuse, recovery and/or recycling potentials (D), relevant
End of life (C1-C4)
scenario information
For the End-of-Life stage two scenarios are considered.
Scenario 1 considers 100% thermal treatment of all raw
Module D includes the credits and loads from the recycling of
materials with heating value including plastic system parts and
the metal components (duplicated in D/1 and D/2) and the
100% recycling of metal system components (C3/1). Landfill of
recycling of the plastic system parts/profiles (D/2). Avoided
all materials without heating value (except metals) including
burdens from the thermal treatment of all raw materials with
glazing (C4/1). Scenario 2 considers 100% recycling of plastic
heating value (including plastic system parts/profiles) (D/1) and
system parts and 100% recycling of metal system components
packaging treatment (duplicated in D/1 and D/2) under
(C3/2). Landfill of all materials without heating value (except
European conditions are considered. This affects only the rate
metals) including glazing (C4/2). Modules C4/1 and C4/2 are
of primary materials (no secondary materials). A waste
identical. The recycling of plastics scenario declared in this
incineration plant with R1-value > 0.6 is assumed.
EPD is currently considered a scenario that is not widely
available in reality due to economic viability limitations
For recycling, a collection rate of 100% is considered.
associated with higher costs of sorting smaller shares of
4 Environmental Product Declaration - Jansen AG - Janisol window width x height: 1230mm x 1480mm
LCA: Results
Results provided in this section are presented in relation to 1 m2 of window type Jansen Janisol (reference dimensions 1230 mm x
1480 mm).
For the End-of-Life stage, two scenarios are considered:
C3/1 - considers 100% recycling of metal system components (duplicated in D/1 and D/2) and 100% thermal treatment of all raw
materials with heating value including plastic system parts.
C3/2 - considers 100% recycling of metal system components (duplicated in D/1 and D/2) and 100% recycling of plastic system parts.
C4/1 and C4/2 - considers landfill of all materials without heating value (except metals) including glazing. Modules C4/1 and C4/2 are
identical.
D/1 - considers credits and loads from the recycling of the metal components (duplicated in D/1 and D/2). Avoided burdens from
packaging treatment (duplicated in D/1 and D/2) and thermal treatment of all raw materials with heating value (including plastic system
parts/profiles) are considered.
D/2 - considers credits and loads from the recycling of the metal components (duplicated in D/1 and D/2) and the recycling of the
plastic system parts/profiles. Avoided burdens from packaging treatment (duplicated in D/1 and D/2) are considered.
DESCRIPTION OF THE SYSTEM BOUNDARY (X = INCLUDED IN LCA; MND = MODULE OR INDICATOR NOT DECLARED; MNR
= MODULE NOT RELEVANT)
Benefits and
Construction loads beyond
Product stage Use stage End of life stage
process stage the system
boundaries
la ire ta m w a Ry lp p u s tro p s n a rT g n iru tc a fu n a M e h t m o rf tro p s n a rTe tis e h t o t e ta g y lb m e s s A e s U e c n a n e tn ia M ria p e R tn e m e c a lp e R tn e m h s ib ru fe R y g re n e la n o ita re p Oe s u re ta w la n o ita re p Oe s u n o itc u rts n o c -e Dn o itilo m e d tro p s n a rT g n is s e c o rp e ts a W la s o p s iD -e s u e R-y re v o c e R-g n ilc y c e Rla itn e to p
A1 A2 A3 A4 A5 B1 B2 B3 B4 B5 B6 B7 C1 C2 C3 C4 D
X X X X X MND MND MNR MNR MNR X MND X X X X X
RESULTS OF THE LCA - ENVIRONMENTAL IMPACT according to EN 15804+A2: 1 m2 Janisol window (44.39 kg/m2)
Parameter Unit A1-A3 A4 A5 B6 C1 C2 C3/1 C3/2 C4/1 C4/2 D/1 D/2
GWP-total kg CO 2 eq 8.3E+01 2.68E-01 5.77E-02 0 0 1.34E-01 8.75E+00 1.46E-01 2.29E-01 2.29E-01 -2.68E+01 -2.59E+01
GWP-fossil kg CO 2 eq 8.28E+01 2.65E-01 9.83E-03 0 0 1.33E-01 8.74E+00 1.46E-01 2.28E-01 2.28E-01 -2.68E+01 -2.58E+01
GWP-
biogenic kg CO 2 eq 2.58E-01 1.12E-03 4.79E-02 0 0 5.6E-04 6.65E-04 3.7E-05 7.67E-04 7.67E-04 -1.82E-02 -2.27E-02
GWP-luluc kg CO 2 eq 2.46E-02 1.48E-03 1.57E-07 0 0 7.41E-04 6.77E-05 5.88E-06 4.2E-04 4.2E-04 -1.24E-03 -1.78E-03
kg CFC11
ODP 4.11E-10 1.59E-14 4.96E-15 0 0 7.96E-15 1.29E-12 5.4E-14 5.35E-13 5.35E-13 -2.2E-11 -1.25E-10
eq
AP mol H+ eq 2.57E-01 2.53E-04 1.08E-05 0 0 1.26E-04 2.34E-03 3.64E-05 1.61E-03 1.61E-03 -6.64E-02 -6.82E-02
EP-
kg P eq 9.05E-05 7.93E-07 1.34E-09 0 0 3.97E-07 3.93E-07 4.03E-08 3.86E-07 3.86E-07 -9.26E-06 -1.44E-05
freshwater
EP-marine kg N eq 7.44E-02 7.88E-05 3.62E-06 0 0 3.94E-05 8.07E-04 1.28E-05 4.13E-04 4.13E-04 -1.07E-02 -1.12E-02
EP-terrestrial mol N eq 8.52E-01 9.47E-04 5.01E-05 0 0 4.73E-04 1.15E-02 1.76E-04 4.54E-03 4.54E-03 -1.01E-01 -1.06E-01
kg NMVOC
POCP 2.2E-01 2.2E-04 9.75E-06 0 0 1.1E-04 2.12E-03 3.45E-05 1.25E-03 1.25E-03 -4.01E-02 -4.55E-02
eq
ADPE kg Sb eq 1.69E-04 2.22E-08 1.21E-10 0 0 1.11E-08 3.17E-08 1.26E-09 2.33E-08 2.33E-08 -4.9E-05 -4.93E-05
ADPF MJ 1.04E+03 3.55E+00 1.36E-02 0 0 1.78E+00 2.51E+00 1E-01 2.98E+00 2.98E+00 -2.85E+02 -3.44E+02
m3 world eq
WDP 5.53E+00 2.38E-03 6.57E-03 0 0 1.19E-03 8.48E-01 2.97E-02 2.5E-02 2.5E-02 -4.56E+00 -5.01E+00
deprived
GWP = Global warming potential; ODP = Depletion potential of the stratospheric ozone layer; AP = Acidification potential of land and water; EP =
Eutrophication potential; POCP = Formation potential of tropospheric ozone photochemical oxidants; ADPE = Abiotic depletion potential for non-fossil
resources; ADPF = Abiotic depletion potential for fossil resources; WDP = Water (user) deprivation potential)
RESULTS OF THE LCA - INDICATORS TO DESCRIBE RESOURCE USE according to EN 15804+A2: 1 m2 Janisol window (44.39
kg/m2)
Parameter Unit A1-A3 A4 A5 B6 C1 C2 C3/1 C3/2 C4/1 C4/2 D/1 D/2
PERE MJ 1.33E+02 2.02E-01 4.78E-01 0 0 1.01E-01 6.49E-01 3.28E-02 4.48E-01 4.48E-01 -2.95E+01 -1.79E+01
PERM MJ 4.75E-01 0 -4.75E-01 0 0 0 0 0 0 0 0 0
PERT MJ 1.34E+02 2.02E-01 3.13E-03 0 0 1.01E-01 6.49E-01 3.28E-02 4.48E-01 4.48E-01 -2.95E+01 -1.79E+01
PENRE MJ 9.37E+02 3.56E+00 1.44E-01 0 0 1.78E+00 1.1E+02 1.08E+02 2.99E+00 2.99E+00 -2.85E+02 -3.44E+02
PENRM MJ 1.08E+02 0 -1.31E-01 0 0 0 -1.08E+02 -1.08E+02 0 0 0 0
PENRT MJ 1.04E+03 3.56E+00 1.36E-02 0 0 1.78E+00 2.51E+00 1E-01 2.99E+00 2.99E+00 -2.85E+02 -3.44E+02
SM kg 1.44E+01 0 0 0 0 0 0 0 0 0 1.17E+01 1.36E+01
RSF MJ 0 0 0 0 0 0 0 0 0 0 0 0
NRSF MJ 0 0 0 0 0 0 0 0 0 0 0 0
FW m3 2.54E-01 2.28E-04 1.55E-04 0 0 1.14E-04 2E-02 6.69E-04 7.58E-04 7.58E-04 -1.61E-01 -1.68E-01
5 Environmental Product Declaration - Jansen AG - Janisol window width x height: 1230mm x 1480mm
PERE = Use of renewable primary energy excluding renewable primary energy resources used as raw materials; PERM = Use of renewable primary
energy resources used as raw materials; PERT = Total use of renewable primary energy resources; PENRE = Use of non-renewable primary energy
excluding non-renewable primary energy resources used as raw materials; PENRM = Use of non-renewable primary energy resources used as raw
materials; PENRT = Total use of non-renewable primary energy resources; SM = Use of secondary material; RSF = Use of renewable secondary fuels;
NRSF = Use of non-renewable secondary fuels; FW = Use of net fresh water
RESULTS OF THE LCA – WASTE CATEGORIES AND OUTPUT FLOWS according to EN 15804+A2:
1 m2 Janisol window (44.39 kg/m2)
Parameter Unit A1-A3 A4 A5 B6 C1 C2 C3/1 C3/2 C4/1 C4/2 D/1 D/2
HWD kg 1.9E-06 1.7E-11 1.33E-12 0 0 8.52E-12 2.48E-10 6.47E-12 1.53E-10 1.53E-10 4.56E-09 -9.26E-07
NHWD kg 3.2E+00 5.1E-04 8.73E-04 0 0 2.55E-04 4.09E-01 1.83E-02 1.53E+01 1.53E+01 1.48E+00 1.56E+00
RWD kg 2.89E-02 4.38E-06 7.77E-07 0 0 2.19E-06 9.17E-05 7.02E-06 3.32E-05 3.32E-05 -7.44E-03 -3.94E-03
CRU kg 0 0 0 0 0 0 0 0 0 0 0 0
MFR kg 6.96E-01 0 0 0 0 0 2.55E+01 2.91E+01 0 0 0 0
MER kg 0 0 0 0 0 0 0 0 0 0 0 0
EEE MJ 0 0 6.59E-02 0 0 0 1.4E+01 1.61E-01 0 0 0 0
EET MJ 0 0 1.18E-01 0 0 0 2.94E+01 3.36E-01 0 0 0 0
HWD = Hazardous waste disposed; NHWD = Non-hazardous waste disposed; RWD = Radioactive waste disposed; CRU = Components for re-use;
MFR = Materials for recycling; MER = Materials for energy recovery; EEE = Exported electrical energy; EET = Exported thermal energy
RESULTS OF THE LCA – additional impact categories according to EN 15804+A2-optional:
1 m2 Janisol window (44.39 kg/m2)
Parameter Unit A1-A3 A4 A5 B6 C1 C2 C3/1 C3/2 C4/1 C4/2 D/1 D/2
Disease
PM 2.41E-06 1.53E-09 5.68E-11 0 0 7.65E-10 1.48E-08 9E-10 1.99E-08 1.99E-08 -8.34E-07 -8.49E-07
incidence
kBq U235
IR 4.66E+00 6.43E-04 1.26E-04 0 0 3.21E-04 1.13E-02 8.42E-04 3.69E-03 3.69E-03 -9.7E-01 -3.69E-01
eq
ETP-fw CTUe 1.25E+03 2.47E+00 6.26E-03 0 0 1.23E+00 1.31E+00 7.33E-02 1.67E+00 1.67E+00 -4.09E+01 -8.81E+01
HTP-c CTUh 5.52E-08 4.97E-11 4.11E-13 0 0 2.48E-11 9.26E-11 2.33E-12 2.55E-10 2.55E-10 -1.08E-08 -1.18E-08
HTP-nc CTUh 1.19E-06 2.57E-09 1.54E-11 0 0 1.29E-09 6.14E-09 8.85E-11 2.82E-08 2.82E-08 -3.31E-07 -3.69E-07
SQP SQP 9.74E+01 1.22E+00 3.95E-03 0 0 6.11E-01 6.75E-01 3.54E-02 6.21E-01 6.21E-01 -8.55E+00 -1.15E+00
PM = Potential incidence of disease due to PM emissions; IR = Potential Human exposure efficiency relative to U235; ETP-fw = Potential comparative
Toxic Unit for ecosystems; HTP-c = Potential comparative Toxic Unit for humans (cancerogenic); HTP-nc = Potential comparative Toxic Unit for humans
(not cancerogenic); SQP = Potential soil quality index
Disclaimer 1 – for the indicator 'Potential Human exposure efficiency relative to U235'.This impact category deals mainly with the
eventual impact of low dose ionizing radiation on human health of the nuclear fuel cycle. It does not consider effects due to possible
nuclear accidents, occupational exposure nor due to radioactive waste disposal in underground facilities. Potential ionizing radiation
from the soil, from radon and from some construction materials is also not measured by this indicator.
Disclaimer 2 – for the indicators 'abiotic depletion potential for non-fossil resources', 'abiotic depletion potential for fossil resources',
'water (user) deprivation potential, deprivation-weighted water consumption', 'potential comparative toxic unit for ecosystems', 'potential
comparative toxic unit for humans – cancerogenic', 'Potential comparative toxic unit for humans - not cancerogenic', 'potential soil
quality index'. The results of this environmental impact indicator shall be used with care as the uncertainties on these results are high
as there is limited experience with the indicator. This EPD was created using a software tool.
References
Standards EN 13115: 2020 Windows - Classification of mechanical
properties - Racking, torsion and operating forces
EN 14351-1
EN 14351-1: 2016, Windows and doors - Product standard, EN 13049
performance characteristics - Part 1: windows and external EN 13049 2003 Windows - Soft and heavy body impact - Test
pedestrian doorsets method, safety requirements and classification
EN 12210
EN 12210: 2016 Windows and doors - Resistance to wind EN 15804
loads - classification EN 15804:2012+A2:2019+AC:2021, Sustainability of
construction works — Environmental Product Declarations —
EN ISO 10140 Core rules for the product category of construction products.
EN ISO 10140-1: 2021 Acoustics - Laboratory measurement of
sound insulation of building elements - Part 1: Application rules ISO 14025
for specific products EN ISO 14025:2011, Environmental labels and declarations —
Type III environmental declarations — Principles and
DIN EN ISO 10077 procedures.
DIN EN ISO 10077-2: 2017 Thermal performance of windows,
doors and shutters - Calculation of thermal transmittance - Part ECHA candidate list
2: Numerical method for frames ECHA candidate list [BSJ1] - Substances of Very High Concern
– SVHC (date 17.01.2023)
EN 12207 Candidate List of substances of very high concern for
EN 12207: 2016 Windows and doors - Air permeability - Authorisation (published in accordance with Article 59(10) of
Classification the REACH Regulation)
EN 13115 REGULATION (EU) No 528/2012
6 Environmental Product Declaration - Jansen AG - Janisol window width x height: 1230mm x 1480mm
REGULATION (EU) No 528/2012 OF THE EUROPEAN LCA-Tool No.: IBU-JAN-202301-LT1-EN
PARLIAMENT AND OF THE COUNCIL Developed by Sphera Solutions GmbH
of 22 May 2012, concerning the making available on the market
and use of biocidal products IBU 2021
Institut
SBR 2011 Bauen und Umwelt e.V.: General Instructions for the EPD
SBR life cycle guide [SBR 2011] programme of Institut Bauen und Umwelt e.V., Version 2.0,
Berlin: Institut Bauen und Umwelt e.V., 2021
Further References www.ibu-epd.com
Sphera LCA FE Software (GaBi ts) PCR Part A
Sphera LCA software (GaBi ts) content update package (CUP) PCR - Part A: Calculation rules for the Life Cycle Assessment
version 2022.2 (https://www.gabi-software.com/support/gabi) and Requirements on the Background Report, version 1.3,
Institut Bauen und Umwelt e.V., 2021.
Sphera LCA Calculator Software (GaBi Envision)
GaBi Envision 5.0 Sphera Solution GmbH, the LCA, EPD and PCR Part B
Ecodesign tool, http://www.gabi- PCR – Part B: Requirements on the EPD for Windows and
software.com/international/software/gabi-envision/, 2022 doors, version 1.6, Institut Bauen und Umwelt e.V., www.bau-
umwelt.com, 2022
Jansen LCA tool
LCA tool for façades, windows & door
7 Environmental Product Declaration - Jansen AG - Janisol window width x height: 1230mm x 1480mm
Publisher
Institut Bauen und Umwelt e.V. +49 (0)30 3087748- 0
Hegelplatz 1 info@ibu-epd.com
10117 Berlin www.ibu-epd.com
Germany
Programme holder
Institut Bauen und Umwelt e.V. +49 (0)30 3087748- 0
Hegelplatz 1 info@ibu-epd.com
10117 Berlin www.ibu-epd.com
Germany
Author of the Life Cycle Assessment
Sphera Solutions GmbH +49 711 341817-0
Hauptstraße 111- 113 info@sphera.com
70771 Leinfelden-Echterdingen www.sphera.com
Germany
Owner of the Declaration
JANSEN AG 0041717639113
Industriestrasse 34 sustainability@jansen.com
9463 Oberriet www.jansen.com
Switzerland
8 Environmental Product Declaration - Jansen AG - Janisol window width x height: 1230mm x 1480mm
