ENVIRONMENTAL PRODUCT DECLARATION
as per ISO 14025 and EN 15804+A2
Owner of the Declaration Kingspan Insulation B.V.
Publisher Institut Bauen und Umwelt e.V. (IBU)
Programme holder Institut Bauen und Umwelt e.V. (IBU)
Declaration number EPD-KIN-20230170-CBA1-EN
Issue date 11/07/2023
Valid to 10/07/2028
Therma™ TW55 R
Kingspan Insulation B.V.
www.ibu-epd.com | https://epd-online.com
General Information
Kingspan Insulation B.V. Therma™ TW55 R
Programme holder Owner of the declaration
IBU – Institut Bauen und Umwelt e.V. Kingspan Insulation B.V.
Hegelplatz 1 Lingewei 8
10117 Berlin 4004LL Tiel
Germany Netherlands
Declaration number Declared product / declared unit
EPD-KIN-20230170-CBA1-EN Therma™ TW55 R
1m2, 70mm thickness, R = 2,55 m2.K/W
D
This declaration is based on the product category rules: Scope:
Insulating materials made of foam plastics, 01/08/2021 The insulation material Therma™ TW55 R is produced by Kingspan
(PCR checked and approved by the SVR) Insulation at the manufacturing facility in Kankaanpää (Finland).
Therma™ TW55 R is an insulation board with a rigid thermoset
Issue date polyisocyanurate (PIR) fibre-free insulation core, faced on both sides with
a coated glass tissue based facing. Therma™ TW55 R is used as thermal
11/07/2023
insulation for timber framing systems.
In order to enable the user of the EPD to calculate the LCA results for
Valid to
different thicknesses, the EPD contains the respective calculation rules.
10/07/2028 The owner of the declaration shall be liable for the underlying information
and evidence; the IBU shall not be liable with respect to manufacturer
information, life cycle assessment data and evidences.
The EPD was created according to the specifications of EN 15804+A2. In
the following, the standard will be simplified as EN 15804.
Verification
The standard EN 15804 serves as the core PCR
Independent verification of the declaration and data according to ISO
14025:2011
Dipl.-Ing. Hans Peters internally X externally
(Chairman of Institut Bauen und Umwelt e.V.)
Florian Pronold Vito D'Incognito,
(Managing Director Institut Bauen und Umwelt e.V.) (Independent verifier)
1 Environmental Product Declaration - Kingspan Insulation B.V. - Therma™ TW55 R
Product
products for buildings - Factory made rigid polyurethane foam
Product description/Product definition (PU) products - Specification.
Therma™ TW55 R is an insulation board with a rigid thermoset The declaration of performance of the product can be found at
polyisocyanurate (PIR) fibre-free insulation core, faced on both www.kingspan.com.
sides with a coated glass tissue based facing. The product is
available in variable thicknesses from 30 mm up to 100 mm. Base materials/Ancillary materials
This EPD is based on a thickness of 70 mm and RD-value of The product contains approximately 1,5 kg/m2 polyurethane
2,55 m²·K/W. For the placing on the market of the product in the rigid foam and 0,6 kg/m2 coated glass tissue based facing.
European Union/European Free Trade Association (EU/EFTA) The main materials of the polyurethane foam are MDI (between
(with the exception of Switzerland) Regulation (EU) No. 57-62 %), polyol (between 27-32 %) and a blowing agent
305/2011 (CPR) applies. The product needs a declaration of (between 5-6 %). Due to the closed cell structure (conform EN
performance taking into consideration EN 13165 - Thermal 13165), the blowing agent remains in the foam. Water, flame
insulation products for buildings - Factory made polyurethane retardants and additives are added (between 4-8 %).
foam (PU) products - Specification and the CE-marking. For the In the current REACH regulations, polyurethane foam
application and use the respective national provisions apply. insulation products are considered “articles” and are
exempt from the requirements of Articles 57 and 59(1)
Application
of REACH Regulation (EC) No 1907/2006. These
Therma™ TW55 R is used as thermal insulation for timber
products are not classified as “hazardous products”
framing systems.
according to any current legislation, and can hence be
declared as follows:
Technical Data
- This article contains substances listed in the
Constructional data candidate list (date: 31.08.2022) exceeding 0.1
Name Value Unit percentage by mass: no.
- This article contains other carcinogenic, mutagenic,
Thermal conductivity according to EN
0.027 W(m.K) reprotoxic (CMR) substances in categories 1A or 1B
13165 for dN < 80mm
which are not on the candidate list, exceeding 0.1
Thermal conductivity according to EN
0.026 W(m.K) percentage by mass: no.
13165 for dN ≥ 80mm
- Biocide products were added to this construction
Reaction to fire according to EN 13165 F
product or it has been treated with biocide products
Compressive strength according to EN CS(10\Y) (this then concerns a treated product as defined by the
13165 100 (EU) Biocidal Products Regulation No. 528/2012
Thickness tolerance according to EN (BPR): no.
T2
13165
Reference service life
Performance data of the product in accordance with the
The reference service life is not to be declared in this
declaration of performance with respect to its essential
EPD as it does not cover the use stage.
characteristics according to EN 13165 - Thermal insulation
LCA: Calculation rules
A4, A5).
Declared Unit
The declared unit (1 m²) and conversion factors are The product stage is a mandatory information module and it
listed in the table below. covers:
Declared unit · A1, raw material extraction and processing, processing of
secondary material input (e.g. recycling processes),
Name Value Unit
· A2, transport to the manufacturer,
Declared unit 1 m2 · A3, manufacturing, including provision of all materials,
Gross density insulation 30 kg/m3 products and energy, packaging processing and its transport,
Grammage 2.1 kg/m2 as well as waste processing up to the end-of-waste state or
disposal of final residues
Layer thickness 0.07 m
during the product stage.
The scope of this EPD is the thermal insulation product
Therma™ TR55R as produced by Kingspan Insulation at the The construction process stage includes:
manufacturing facility in Kankaanpää (Finland). The · A4 transport to the building site;
environmental impacts have been calculated over the calendar · A5 installation in the building including provision of all
year 2021. materials, products and energy, as well as waste processing up
to the end-of-waste state or disposal of final residues during the
The EPD is studied for a product thickness of 70 mm. construction process stage.
Multiplication factors are included to calculate impacts for other
product thicknesses within the range of 30 to 100 mm. The end-of-life stage is a mandatory information module and it
covers:
· C1 de-construction, demolition;
System boundary
· C2 transport to waste processing;
The type of EPD according to EN 15804 is: · C3 waste processing for reuse, recovery and/or recycling;
cradle to gate with options, modules C1–C4, and · C4 disposal (not applicable for this EPD) including provision
module D (A1–A3, C, D and additional modules: and all transport, provision of all materials, products and related
2 Environmental Product Declaration - Kingspan Insulation B.V. - Therma™ TW55 R
energy and water use. Basically, a comparison or an evaluation of EPD data is only
possible if all the data sets to be compared were created
Environmental burden of the incineration (R1 > 60 %) of the according to EN 15804 and the building context, respectively
product the product-specific characteristics of performance, are taken
at the end-of-life stage are assigned to the product system into account.
(C3); resulting potential credits for thermal and electrical energy
from energy substitution are declared in module D. Background database
Background data from GaBi ts Version 10 is used with
Geographic Representativeness GaBi data sets CUP2022.1.
Land or region, in which the declared product system is
manufactured, used or handled at the end of the product´s
lifespan: Europe Period under review
The input data for raw material production and the consumption
of process energy on the manufacturing facility was measure
Comparability
data during January 1st 2021 to December 31st 2021, i.e.
collected over a 12 month period.
LCA: Scenarios and additional technical information
Installation into the building (A5)
Characteristic product properties of biogenic carbon
The total mass of biogenic carbon containing materials is less Name ValueUnit
than 5 % of the total mass of the product and accompanying Output substances following waste treatment on
0.062 kg
packaging. site
The recycling of the packaging is considered in A5.
Technical information
The following technical information is a basis for the
declared modules or can be used for developing End of life (C1-C4)
specific scenarios in the context of a building The assumptions for C1 are: diesel driven excavator (100 kW;
assessment. 0.2 litre fuel per ton excavated material). The assumptions for
C2 are: Truck Euro 6, diesel driven, 26-28 t gross weight,
Manufacturing (A3) assumed distance 50 km
A polyethylene packaging foil is used. The products Name Value Unit
are transported on wooden pallets.
Collected as mixed construction waste 2.1 kg
Within Module A3 the following packaging of the final
Energy recovery 2.1 kg
product is included:
- Polyethylene cover and wrap: 0,022 kg/m² Reuse, recovery and/or recycling potentials (D), relevant
- Wooden pallet: 0,040 kg/m² scenario information
Waste incineration with energy recuperation is assumed as
Transport to the building site (A4)
end-of-life scenario
Name Value Unit
Litres of fuel 0.0103 l/100km
Transport distance 100 km
Gross density of products transported 30 kg/m3
3 Environmental Product Declaration - Kingspan Insulation B.V. - Therma™ TW55 R
LCA: Results
DESCRIPTION OF THE SYSTEM BOUNDARY (X = INCLUDED IN LCA; ND = MODULE OR INDICATOR NOT DECLARED; MNR =
MODULE NOT RELEVANT)
Benefits and
Construction loads beyond
Product stage Use stage End-of-life stage
process stage the system
boundaries
la ire ta m w a Ry lp p u s tro p s n a rT g n iru tc a fu n a M e h t m o rf tro p s n a rTe tis e h t o t e ta g y lb m e s s A e s U e c n a n e tn ia M ria p e R tn e m e c a lp e R tn e m h s ib ru fe R y g re n e la n o ita re p Oe s u re ta w la n o ita re p Oe s u n o itc u rts n o c -e Dn o itilo m e d tro p s n a rT g n is s e c o rp e ts a W la s o p s iD -e s u e R-y re v o c e R-g n ilc y c e Rla itn e to p
A1 A2 A3 A4 A5 B1 B2 B3 B4 B5 B6 B7 C1 C2 C3 C4 D
X X X X X MND MND MNR MNR MNR MND MND X X X X X
RESULTS OF THE LCA - ENVIRONMENTAL IMPACT according to EN 15804+A2: 1m2 70mm Therma™ TW55 R
Parameter Unit A1-A3 A4 A5 C1 C2 C3 C4 D
GWP-total kg CO 2 eq 5.02E+00 1.77E-02 1.27E-01 1.35E-03 8.84E-03 3.88E+00 0 -1.53E+00
GWP-fossil kg CO 2 eq 5.09E+00 1.76E-02 5.62E-02 1.35E-03 8.8E-03 3.88E+00 0 -1.52E+00
GWP-biogenic kg CO 2 eq -7.57E-02 -2.43E-05 7.12E-02 1.8E-06 -1.22E-05 2.81E-04 0 -7.79E-03
GWP-luluc kg CO 2 eq 4.28E-03 9.82E-05 7.91E-07 1.66E-08 4.91E-05 2.76E-05 0 -1.67E-04
ODP kg CFC11 eq 4.9E-12 1.06E-15 1.52E-14 8.25E-17 5.28E-16 3.73E-13 0 -1.03E-11
AP mol H+ eq 1.18E-02 1.81E-05 1.7E-05 6.25E-06 9.07E-06 2.09E-03 0 -2E-03
EP-freshwater kg P eq 1.89E-05 5.26E-08 3.77E-09 2.71E-10 2.63E-08 1.96E-07 0 -2.1E-06
EP-marine kg N eq 2.86E-03 5.94E-06 5.17E-06 2.98E-06 2.97E-06 9.9E-04 0 -5.44E-04
EP-terrestrial mol N eq 3.02E-02 7.07E-05 7.96E-05 3.26E-05 3.53E-05 1.15E-02 0 -5.82E-03
kg NMVOC
POCP 1.25E-02 1.6E-05 1.43E-05 8.45E-06 7.99E-06 2.55E-03 0 -1.52E-03
eq
ADPE kg Sb eq 4.74E-06 1.47E-09 3.71E-10 5.51E-11 7.36E-10 1.02E-08 0 -2.3E-07
ADPF MJ 1.26E+02 2.35E-01 3.53E-02 1.82E-02 1.18E-01 1.2E+00 0 -2.59E+01
m3 world eq
WDP 7.2E-01 1.58E-04 1.27E-02 2.5E-06 7.9E-05 4.24E-01 0 -1.62E-01
deprived
GWP = Global warming potential; ODP = Depletion potential of the stratospheric ozone layer; AP = Acidification potential of land and water; EP =
Eutrophication potential; POCP = Formation potential of tropospheric ozone photochemical oxidants; ADPE = Abiotic depletion potential for non-fossil
resources; ADPF = Abiotic depletion potential for fossil resources; WDP = Water (user) deprivation potential)
RESULTS OF THE LCA - INDICATORS TO DESCRIBE RESOURCE USE according to EN 15804+A2: 1m2 70mm Therma™ TW55
R
Parameter Unit A1-A3 A4 A5 C1 C2 C3 C4 D
PERE MJ 1E+01 1.34E-02 6.04E-01 6.88E-05 6.69E-03 2.29E-01 0 -7.11E+00
PERM MJ 5.96E-01 0 -5.96E-01 0 0 0 0 0
PERT MJ 1.06E+01 1.34E-02 8.68E-03 6.88E-05 6.69E-03 2.29E-01 0 -7.11E+00
PENRE MJ 6.1E+01 2.36E-01 9.86E-01 1.83E-02 1.18E-01 6.58E+01 0 -2.59E+01
PENRM MJ 6.55E+01 0 -9.5E-01 0 0 -6.46E+01 0 0
PENRT MJ 1.26E+02 2.36E-01 3.53E-02 1.83E-02 1.18E-01 1.2E+00 0 -2.59E+01
SM kg 0 0 0 0 0 0 0 0
RSF MJ 0 0 0 0 0 0 0 0
NRSF MJ 0 0 0 0 0 0 0 0
FW m3 3.42E-02 1.51E-05 2.99E-04 1.04E-07 7.57E-06 9.98E-03 0 -6.84E-03
PERE = Use of renewable primary energy excluding renewable primary energy resources used as raw materials; PERM = Use of renewable primary
energy resources used as raw materials; PERT = Total use of renewable primary energy resources; PENRE = Use of non-renewable primary energy
excluding non-renewable primary energy resources used as raw materials; PENRM = Use of non-renewable primary energy resources used as raw
materials; PENRT = Total use of non-renewable primary energy resources; SM = Use of secondary material; RSF = Use of renewable secondary fuels;
NRSF = Use of non-renewable secondary fuels; FW = Use of net fresh water
RESULTS OF THE LCA – WASTE CATEGORIES AND OUTPUT FLOWS according to EN 15804+A2:
1m2 70mm Therma™ TW55 R
Parameter Unit A1-A3 A4 A5 C1 C2 C3 C4 D
HWD kg 3.84E-08 1.13E-12 3.14E-12 6.03E-14 5.65E-13 1.45E-10 0 -3.51E-09
NHWD kg 1.45E-01 3.38E-05 5.48E-03 1.71E-06 1.69E-05 2.24E-01 0 -1.31E-02
RWD kg 2.52E-03 2.91E-07 1.73E-06 2E-08 1.45E-07 5.13E-05 0 -2.04E-03
CRU kg 0 0 0 0 0 0 0 0
MFR kg 0 0 0 0 0 0 0 0
MER kg 0 0 6.18E-02 0 0 2.1E+00 0 0
EEE MJ 0 0 2.04E-01 0 0 6.64E+00 0 0
EET MJ 0 0 3.66E-01 0 0 1.2E+01 0 0
4 Environmental Product Declaration - Kingspan Insulation B.V. - Therma™ TW55 R
HWD = Hazardous waste disposed; NHWD = Non-hazardous waste disposed; RWD = Radioactive waste disposed; CRU = Components for re-use;
MFR = Materials for recycling; MER = Materials for energy recovery; EEE = Exported electrical energy; EET = Exported thermal energy
RESULTS OF THE LCA – additional impact categories according to EN 15804+A2-optional:
1m2 70mm Therma™ TW55 R
Parameter Unit A1-A3 A4 A5 C1 C2 C3 C4 D
Disease
PM 1.03E-07 1.05E-10 1.34E-10 7.08E-11 5.24E-11 8.57E-09 0 -1.66E-08
incidence
IR kBq U235 eq 2.79E-01 4.26E-05 2.61E-04 2.91E-06 2.13E-05 8.12E-03 0 -3.45E-01
ETP-fw CTUe 5.1E+01 1.63E-01 2.12E-02 1.27E-02 8.17E-02 5.44E-01 0 -5.69E+00
HTP-c CTUh 3.67E-09 3.29E-12 1.27E-12 2.34E-13 1.65E-12 3.23E-11 0 -2.61E-10
HTP-nc CTUh 2.7E-07 1.71E-10 9.84E-11 1.19E-11 8.54E-11 1.46E-09 0 -1E-08
SQP SQP 3E+01 8.1E-02 9.61E-03 5.02E-05 4.05E-02 2.81E-01 0 -4.62E+00
PM = Potential incidence of disease due to PM emissions; IR = Potential Human exposure efficiency relative to U235; ETP-fw = Potential comparative
Toxic Unit for ecosystems; HTP-c = Potential comparative Toxic Unit for humans (cancerogenic); HTP-nc = Potential comparative Toxic Unit for humans
(not cancerogenic); SQP = Potential soil quality index
Disclaimer 1 – for the indicator 'Potential Human exposure efficiency relative to U235'.This impact category deals mainly with the
eventual impact of low-dose ionizing radiation on human health of the nuclear fuel cycle. It does not consider effects due to possible
nuclear accidents, occupational exposure or to radioactive waste disposal in underground facilities. Potential ionizing radiation from the
soil, radon and from some construction materials is also not measured by this indicator.
Disclaimer 2 – for the indicators 'abiotic depletion potential for non-fossil resources', 'abiotic depletion potential for fossil resources',
'water (user) deprivation potential, deprivation-weighted water consumption', 'potential comparative toxic unit for ecosystems', 'potential
comparative toxic unit for humans – cancerogenic', 'Potential comparative toxic unit for humans - not cancerogenic', 'potential soil
quality index'. The results of this environmental impact indicator shall be used with care as the uncertainties on these results are high
as there is limited experience with the indicator.
Factors for different thicknesses
The LCA results for the insulation material declared in this EPD refer to a product with a thickness of 70 mm. To enable the user of the
EPD to calculate the results for different thicknesses the factors in the following table can be used for the calculation. The LCA results
in chapter 5 have to be multiplied with these factors.
This EPD was created using a software tool.
References
Biocidal Products Regulation No. 528/2012 (BPR) EN 13165
Regulation (EU) No 528/2012 of the European EN 13165:2012+A2:2016: Thermal insulation products
Parliament and of the Council of 22 May 2012 for buildings. Factory made polyurethane foam (PU)
concerning the making available on the market and products. Specification
use of biocidal products
EN 15804
CPR EN 15804:2012+A2:2019+AC:2021, Sustainability of
Regulation (EU) No. 305/2011 of the European construction works — Environmental Product
Parliament and of the Council of 9 March 2011 laying Declarations — Core rules for the product category of
down harmonised condition for the marketing of construction products.
construction products and repealing Council Directive
89/106/EC GaBi ts
thinkstep AG: Leinfelden-Echterdingen GaBi Software-
ISO 14025 System and Database for Life Cycle Engineering 1992-
EN ISO 14025:2011, Environmental labels and 2019
declarations — Type III environmental declarations —
Principles and procedures. IBU 2021
Institut Bauen und Umwelt e.V.: General Instructions
5 Environmental Product Declaration - Kingspan Insulation B.V. - Therma™ TW55 R
for the EPD programme of Institut Bauen und Umwelt PCR 2023, Part B
e.V., Version 2.0, Berlin: Institut Bauen und Umwelt Institut Bauen und Umwelt e.V., Berlin (pub.): Product
e.V., 2021. Category Rules for Construction Products from the
www.ibu-epd.com range of Environmental Product Declarations of Institut
Bauen und Umwelt (IBU), Part B: Requirements on the
LCA-tool EPD for insulating materials made of foam
Kingspan LCA tool, version 1.1. IBU-KSI-202001-LT1- plastics. May 2023.
EN.
Developed by Sphera Solutions GmbH (formely REACH
Thinkstep GmbH) Regulation (EC) No 1907/2006 of the European
Parliament and of the Council on the Registration,
PCR Version 1.7, Part A Evaluation, Authorisation and Restriction of Chemicals
Institut Bauen und Umwelt e.V., Berlin (pub.): Product (REACH)
Category Rules for Building-Related Products and https://echa.europa.eu/candidate-list-table;
services, Part A: Calculation Rules for the Life Cycle
Assessment and Requirements on the Project Report Candidate list
according to EN 15804+A2:2019 https://echa.europa.eu/candidate-list-table; accessed
November 2021 31.08.2022, 233 substances listed.
6 Environmental Product Declaration - Kingspan Insulation B.V. - Therma™ TW55 R
Publisher
Institut Bauen und Umwelt e.V. +49 (0)30 3087748- 0
Hegelplatz 1 info@ibu-epd.com
10117 Berlin www.ibu-epd.com
Germany
Programme holder
Institut Bauen und Umwelt e.V. +49 (0)30 3087748- 0
Hegelplatz 1 info@ibu-epd.com
10117 Berlin www.ibu-epd.com
Germany
Author of the Life Cycle Assessment
Kingspan Insulation B.V. +31 (0) 543 543 210
Lingewei 8 info@kingspaninsulation.nl
4004LL Tiel www.kingspan.com
Netherlands
Owner of the Declaration
Kingspan Insulation B.V. +31 (0) 543 543 210
Lingewei 8 info@kingspaninsulation.nl
4004LL Tiel www.kingspan.com
Netherlands
7 Environmental Product Declaration - Kingspan Insulation B.V. - Therma™ TW55 R
