ENVIRONMENTAL PRODUCT DECLARATION
as per ISO 14025 and EN 15804+A2
Owner of the Declaration VELUX Group
Publisher Institut Bauen und Umwelt e.V. (IBU)
Programme holder Institut Bauen und Umwelt e.V. (IBU)
Declaration number EPD-VEL-20230049-IBA2-EN
Issue date 11.05.2023
Valid to 10.05.2028
Window operator for VELUX pivot hinged windows and KSX 100K
(for retrofitting), solar powered
VELUX Group
www.ibu-epd.com | https://epd-online.com
General Information
VELUX Group Window operator for VELUX pivot hinged windows
and KSX 100K (for retrofitting), solar powered
Programme holder Owner of the declaration
IBU – Institut Bauen und Umwelt e.V. VELUX Group
Hegelplatz 1 Ådalsvej 99
10117 Berlin 2970 Hørsholm
Germany Denmark
Declaration number Declared product / declared unit
EPD-VEL-20230049-IBA2-EN The declared unit is one piece of electrical window operator.
This declaration is based on the product category rules: Scope:
Drive systems for automatic doors and gates, 01.08.2021 The EPD is a specific EPD covering VELUX electrical window operator for
(PCR checked and approved by the SVR) the solar powered pivot hinged windows and window openor KSX 100K for
retrofitting. The operator consists of a chain operator, a rain sensor, a solar
panel and a remote. The products are manufactured by the VELUX Group
Issue date at a production site in the Czech Republic.
The owner of the declaration shall be liable for the underlying information
11.05.2023
and evidence; the IBU shall not be liable with respect to manufacturer
information, life cycle assessment data and evidences.
Valid to
The EPD was created according to the specifications of EN 15804+A2. In
10.05.2028 the following, the standard will be simplified as EN 15804.
Verification
The standard EN 15804 serves as the core PCR
Independent verification of the declaration and data according to ISO
14025:2011
internally X externally
Dipl.-Ing. Hans Peters
(Chairman of Institut Bauen und Umwelt e.V.)
Florian Pronold Dr.-Ing. Nikolay Minkov,
(Managing Director Institut Bauen und Umwelt e.V.) (Independent verifier)
1 Environmental Product Declaration - VELUX Group - Window operator for VELUX pivot hinged windows and KSX 100K (for retrofitting), solar powered
Product
Product description/Product definition Base materials/Ancillary materials
EPD covering VELUX electrical window operator for the solar
Product content
powered pivot hinged windows and KXS 100K. The operator
Name Value Unit
consists of a chain operator including a battery, a solar panel, a
rain sensor and a remote. The products are manufactured by Other plastic components 43 %
the VELUX Group at a production site in the Czech Republic. Battery 20 %
For the placing on the market of the product in the European Other metal components 18 %
Union/European Free Trade Association (EU/EFTA) (with the
Solar cell 8 %
exception of Switzerland) Regulation (EU) No. 305/2011 (CPR)
PCBA 4 %
applies. The products are in compliance with the Machinery
Directive 2006/42/EC, the Radio Equipment Directive Motor 4 %
2014/53/EU and the RoHS Directive 2011/65/EU. A declaration Cables 2 %
of conformity is available from the manufacturer. Other (paper and silicone) 1 %
Application Packaging materials include 0,36 kg cardboard and paper, 0,14
The VELUX solar powered window operator is either installed in kg polystyrene (EPS) and 0,03 kg low density polyethylen
new windows before distribution to customers or it is sold (LDPE).
separately for retrofitting.
This product/article/at least one partial article contains
Technical Data substances listed in the candidate list (date: 08.06.2022)
The CE marking for solar powered window operators does not exceeding 0.1 percentage by mass: NO.
specify the need for a Declaration of Performance. Instead, a
Reference service life
Declaration of Conformity is required.
No reference service life (RSL) is defined for the operators as
The performance values relevant for the product are specified
the use stage modules are not included in the EPD. There is no
in the table below.
generally acknowledged or common way to assess the RSL for
Constructional data
this type of product. Furthermore, the lifetime of the products
Name Value Unit depends greatly on the use pattern and environmental
Protection class IP 44 class conditions in use, which differs for different users and which is
difficult to predict at the time of sale.
Sound pressure level LpA ≤70 dB(A)
LCA: Calculation rules
components to the manufacturing sites
Declared Unit
The declared unit is one piece. This corresponds to an A3 - Manufacturing: The products are produced/assembled at
electrical window operator system, including a chain operator, a the VELUX production site, where the finished window operator
solar panel, a rain sensor and a remote. is ready for shipment.
Name Value Unit End of life stage:
Declared unit 1 pce.
C1 - De-construction/demolition: de-construction of the product
Weight 1,71 kg
with the use of manual hand tools.
Conversion factor to kg 0,58 -
Other declared units are allowed if the conversion is shown C2 - Transport: transport of the product to waste treatment
transparently. including to and from sorting and shredding facilities.
A data quality and a sensitivity analysis show that the results C3 - Waste processing: includes sorting, shredding, incineration
are robust with regard to data quality and appropriateness. and recycling processes.
There is low variability of production processes and product
variations have a limited influence on the results. C4 - Disposal: disposal of all materials
System boundary
Benefits and loads beyond the system boundaries:
Type of EPD:
Cradle to gate - with options. The following life cycle phases D - Reuse, recovery and recycling potential: benefits from
were considered: plastic incineration processes and material recycling. End of life
includes all activities from when the product reaches the end of
Product stage: its service life and no longer provides any functionality until all
materials and components are processed for
A1 - Raw material supply: extraction and processing, reuse/recycling/energy recovery or are disposed of.
production of the pre-products (e.g. motor suspension, PCB,
battery...). Production of sales packaging: cardboard boxes, The applied end-of-life scenario follows the requirements in the
paper labels, EPS and plastic film. PCR Part A, chapter 6.2 regarding complex products, with a
combination of recycling, thermal waste treatment and
A2 - Transport: Transport of pre-products and packaging landfilling. 100% of the material is considered in the end of life
2 Environmental Product Declaration - VELUX Group - Window operator for VELUX pivot hinged windows and KSX 100K (for retrofitting), solar powered
scenario. Generally metals, cables, batteries and
polychlorinated byphenyl (PCB)'s are recycled, plastic parts are Comparability
incinerated with energy recovery whereas magnets and the Basically, a comparison or an evaluation of EPD data is only
solar cell are landfilled. possible if all the data sets to be compared were created
according to EN 15804 and the building context, respectively
Geographic Representativeness the product-specific characteristics of performance, are taken
Land or region, in which the declared product system is into account. The used background software and database is
manufactured, used or handled at the end of the product´s GaBi (DB version 2021.2)
lifespan: Europe
LCA: Scenarios and additional technical information
No Reference Service Life (RFL) is declared, because the use
Characteristic product properties of biogenic carbon stage modules are not declared.
The product does not contain biogenic carbon.
End of life (C1-C4)
Information on describing the biogenic Carbon Content at
Name Value Unit
factory gate
Collected separately waste type Electronics 1.7 kg
Name ValueUnit
Recycling 0.81 kg
kg
Biogenic carbon content in product - Energy recovery 0.74 kg
C
Landfilling 0.16 kg
Biogenic carbon content in accompanying kg
0.29
packaging C
Reuse, recovery and/or recycling potentials (D), relevant
scenario information
Name Value Unit
Replaced materials 0.17 kg
Assembly (A5) Replaced thermal energy 4.2 MJ
Name Value Unit Replaced electricity 2.3 MJ
Cardboard for recycling 0.36 kg
EPS packaging for incineration 0.14 kg
Plastic packaging for incineration (PE) 0.03 kg
3 Environmental Product Declaration - VELUX Group - Window operator for VELUX pivot hinged windows and KSX 100K (for retrofitting), solar powered
LCA: Results
DESCRIPTION OF THE SYSTEM BOUNDARY (X = INCLUDED IN LCA; MND = MODULE OR INDICATOR NOT DECLARED; MNR
= MODULE NOT RELEVANT)
Benefits and
Construction loads beyond
Product stage Use stage End of life stage
process stage the system
boundaries
la ire ta m w a Ry lp p u s tro p s n a rT g n iru tc a fu n a M e h t m o rf tro p s n a rTe tis e h t o t e ta g y lb m e s s A e s U e c n a n e tn ia M ria p e R tn e m e c a lp e R tn e m h s ib ru fe R y g re n e la n o ita re p Oe s u re ta w la n o ita re p Oe s u n o itc u rts n o c -e Dn o itilo m e d tro p s n a rT g n is s e c o rp e ts a W la s o p s iD -e s u e R-y re v o c e R-g n ilc y c e Rla itn e to p
A1 A2 A3 A4 A5 B1 B2 B3 B4 B5 B6 B7 C1 C2 C3 C4 D
X X X MND MND MND MND MNR MNR MNR MND MND X X X X X
RESULTS OF THE LCA - ENVIRONMENTAL IMPACT according to EN 15804+A2: 1 pcs window operator
Parameter Unit A1 A2 A3 C1 C2 C3 C4 D
GWP-total kg CO 2 eq 2.01E+01 4.44E-01 8.33E-01 0 8.75E-03 1.17E+00 3.05E-03 -1.25E+00
GWP-fossil kg CO 2 eq 2.05E+01 4.43E-01 1.28E+00 0 8.69E-03 1.17E+00 3.13E-03 -1.24E+00
GWP-biogenic kg CO 2 eq -3.85E-01 1.96E-04 -4.45E-01 0 -1.11E-05 7.21E-05 -9.09E-05 -3.81E-05
GWP-luluc kg CO 2 eq 3.1E-02 1.2E-03 9.43E-04 0 7.12E-05 -3.8E-05 9.19E-06 -1.47E-03
ODP kg CFC11 eq 1.26E-05 4.91E-17 1.83E-11 0 1.11E-18 -3.02E-08 1.22E-17 -6.99E-15
AP mol H+ eq 3.59E-01 1.13E-02 3.65E-03 0 2.72E-05 7.6E-04 2.23E-05 -4.05E-03
EP-freshwater kg P eq 5.4E-03 5.01E-07 1.28E-05 0 2.58E-08 -3.44E-05 5.25E-09 -1.22E-06
EP-marine kg N eq 1.94E-01 3.09E-03 1.09E-03 0 1.25E-05 4.77E-04 5.78E-06 -6.71E-04
EP-terrestrial mol N eq 2.4E-01 3.39E-02 1.12E-02 0 1.4E-04 6.2E-03 6.35E-05 -7.24E-03
kg NMVOC
POCP 8.37E-02 8.46E-03 3.27E-03 0 2.45E-05 9.94E-04 1.75E-05 -2.01E-03
eq
ADPE kg Sb eq 9.17E-04 2E-08 1.73E-07 0 6.62E-10 -9.64E-08 2.95E-10 -4.03E-05
ADPF MJ 2.99E+02 5.53E+00 2.6E+01 0 1.16E-01 -1.34E+00 4.15E-02 -1.71E+01
m3 world eq
WDP 2.38E+01 1.72E-03 1.53E-01 0 7.55E-05 1.48E-01 3.36E-04 -2.62E-01
deprived
GWP = Global warming potential; ODP = Depletion potential of the stratospheric ozone layer; AP = Acidification potential of land and water; EP =
Eutrophication potential; POCP = Formation potential of tropospheric ozone photochemical oxidants; ADPE = Abiotic depletion potential for non-fossil
resources; ADPF = Abiotic depletion potential for fossil resources; WDP = Water (user) deprivation potential)
RESULTS OF THE LCA - INDICATORS TO DESCRIBE RESOURCE USE according to EN 15804+A2: 1 pcs window operator
Parameter Unit A1 A2 A3 C1 C2 C3 C4 D
PERE MJ 7.18E+01 1.21E-01 1.35E+01 0 6.46E-03 3.8E-01 5.59E-03 -3.66E+00
PERM MJ 0 0 0 0 0 0 0 0
PERT MJ 7.18E+01 1.21E-01 1.35E+01 0 6.46E-03 3.8E-01 5.59E-03 -3.66E+00
PENRE MJ 2.9E+02 5.54E+00 1.79E+01 0 1.16E-01 1.33E+01 4.15E-02 -1.71E+01
PENRM MJ 1.51E+01 0 8.12E+00 0 0 -1.47E+01 0 0
PENRT MJ 3.05E+02 5.54E+00 2.6E+01 0 1.16E-01 -1.34E+00 4.15E-02 -1.71E+01
SM kg 1.77E-01 0 0 0 0 0 0 0
RSF MJ 0 0 0 0 0 0 0 0
NRSF MJ 0 0 0 0 0 0 0 0
FW m3 5.68E-01 1.44E-04 7.05E-03 0 7.39E-06 3.71E-03 1.02E-05 -1.09E-02
PERE = Use of renewable primary energy excluding renewable primary energy resources used as raw materials; PERM = Use of renewable primary
energy resources used as raw materials; PERT = Total use of renewable primary energy resources; PENRE = Use of non-renewable primary energy
excluding non-renewable primary energy resources used as raw materials; PENRM = Use of non-renewable primary energy resources used as raw
materials; PENRT = Total use of non-renewable primary energy resources; SM = Use of secondary material; RSF = Use of renewable secondary fuels;
NRSF = Use of non-renewable secondary fuels; FW = Use of net fresh water
RESULTS OF THE LCA – WASTE CATEGORIES AND OUTPUT FLOWS according to EN 15804+A2:
1 pcs window operator
Parameter Unit A1 A2 A3 C1 C2 C3 C4 D
HWD kg 1.9E-03 1.26E-10 1.35E-04 0 5.84E-12 3.89E-10 4.41E-12 -2.57E-09
NHWD kg 3.65E-01 6.5E-04 3.15E-02 0 1.72E-05 3.19E-01 2.07E-01 -5.06E-02
RWD kg 2.58E-03 6.35E-06 1.27E-03 0 1.4E-07 1.45E-04 4.36E-07 -7.74E-04
CRU kg 0 0 0 0 0 0 0 0
MFR kg 0 0 0 0 0 6.07E-01 0 0
MER kg 0 0 0 0 0 6.17E-01 0 0
EEE MJ 0 0 0 0 0 0 0 2.18E+00
EET MJ 0 0 0 0 0 0 0 3.93E+00
4 Environmental Product Declaration - VELUX Group - Window operator for VELUX pivot hinged windows and KSX 100K (for retrofitting), solar powered
HWD = Hazardous waste disposed; NHWD = Non-hazardous waste disposed; RWD = Radioactive waste disposed; CRU = Components for re-use;
MFR = Materials for recycling; MER = Materials for energy recovery; EEE = Exported electrical energy; EET = Exported thermal energy
RESULTS OF THE LCA – additional impact categories according to EN 15804+A2-optional:
1 pcs window operator
Parameter Unit A1 A2 A3 C1 C2 C3 C4 D
Disease
PM 6.93E+02 3.9E+00 9.09E+00 0 8.12E-02 7.82E-01 2.22E-02 -4.08E+00
incidence
IR kBq U235 eq 8.37E+02 6.85E-02 2.4E+01 0 1.57E-03 -1.58E+00 1.27E-03 -1.73E+00
ETP-fw CTUe 8.38E+00 3.53E-02 7.35E-02 0 7.8E-04 -6.1E-02 1.8E-04 -4.14E-02
HTP-c CTUh 1.75E-19 1.31E-21 4.63E-20 0 2.9E-23 3.72E-20 3.82E-23 -2.19E-19
HTP-nc CTUh 4.02E-08 7.5E-11 1.83E-10 0 1.65E-12 5.31E-10 3.39E-12 -8.87E-10
SQP SQP 7.66E-08 1.69E-12 8.27E-11 0 3.86E-14 -1.26E-10 1.02E-13 -3.59E-10
PM = Potential incidence of disease due to PM emissions; IR = Potential Human exposure efficiency relative to U235; ETP-fw = Potential comparative
Toxic Unit for ecosystems; HTP-c = Potential comparative Toxic Unit for humans (cancerogenic); HTP-nc = Potential comparative Toxic Unit for humans
(not cancerogenic); SQP = Potential soil quality index
Disclaimer 1 – for the indicator “Potential Human exposure efficiency relative to U235”. This impact category deals mainly with the
eventual impact of low-dose ionizing radiation on human health of the nuclear fuel cycle. It does not consider effects due to possible
nuclear accidents, occupational exposure or radioactive waste disposal in underground facilities. Potential ionizing radiation from the
soil, radon and from some construction materials is also not measured by this indicator.
Disclaimer 2 – for the indicators “abiotic depletion potential for non-fossil resources”, “abiotic depletion potential for fossil resources”,
“water (user) deprivation potential, deprivation-weighted water consumption”, “potential comparative toxic unit for ecosystems”,
“potential comparative toxic unit for humans – cancerogenic”, “Potential comparative toxic unit for humans - not cancerogenic”,
“potential soil quality index”. The results of this environmental impact indicator shall be used with care as the uncertainties on these
results are high as there is limited experience with the indicator.
References
IBU PCR Part A Directive 2006/42/EC
IBU PCR Part A: Institut Bauen und Umwelt e.V., Product Directive 2006/42/EC of the European Parliament and of the
Category Rules for Building-Related Products and Services. Council, 17 May 2006 on Machinery.
Calculation Rules for the Life Cycle Assessment and
Requirements on the Project Report according to EN EN 14351-1:2006+A2:2016
15804+A2:2019. EN14351-1:2006+A2:2016, Windows and doors - Product
standard, performance characteristics - Part 1: Windows and
external pedestrian doorsets.
IBU PCR Part B
IBU PCR Part B: Institut Bauen und Umwelt e.V., Requirements EN 15804:2019+A2
on the EPD for Drive systems for automatic doors and gates, EN15804:2019+A2: Sustainability of construction works -
version 1.6. Environmental Product Declarations - Core rules for the product
category of construction products.
IBU 2021
IBU 2021: Institut Bauen und Umwelt e.V.: General Instructions Directive 2014/53/EU
for the EPD programme of Institut Bauen und Umwelt e.V. Directive 2014/53/EU of the European Parliament and of the
Version 2.0, Berlin: Institut Bauen und Umwelt e.V., 2021. Council of 16 April 2014 on the harmonisation of the laws of the
www.ibu-epd.com. Member States relating to the making available on the market
of radio equipment.
EN 13501-1
EN13501-1, 2018: Fire classification of construction products Directive 2011/65/EU
and building elements - Part 1: Classification using data from Directive 2011/65/EU of the European Parliament and of the
reaction to fire tests. Council of 8 June 2011 on the restriction of the use of certain
hazardous substances in electrical and electronic equipment.
DIN EN ISO 14025:2011-10
DIN EN ISO 14025:2011-10, Environmental labels and Directive 2006/42/EC
declarations - Type III environmental declarations - Principles Directive 2006/42/EC of the European Parliament and of the
and procedures. Council of 17 May 2006 on machinery.
Regulation (EU) No 305/2011 Candidate list
Regulation (EU) No 305/2011 of the European Parliament and Candidate List of substances of very high concern for
of the Council, 9 March 2011, Laying down harmonised Authorisation, (date: 08.06.2022).
conditions for the marketing of constructional products.
GaBi LCA software and database
Directive 2011/65/EU The LCA modelling software is GaBi program version
Directive 2011/65/EU of the European Parliament and of the 10.5.1.124 with corresponding databases from Sphera
Council, 8 June 2011, on the restriction of the use of certain Solutions GmbH. Documentation hyperlink www.gabi-
hazardous substances in electrical and electronic equipment. software.com/support/gabi.
5 Environmental Product Declaration - VELUX Group - Window operator for VELUX pivot hinged windows and KSX 100K (for retrofitting), solar powered
Publisher
Institut Bauen und Umwelt e.V. +49 (0)30 3087748- 0
Hegelplatz 1 info@ibu-epd.com
10117 Berlin www.ibu-epd.com
Germany
Programme holder
Institut Bauen und Umwelt e.V. +49 (0)30 3087748- 0
Hegelplatz 1 info@ibu-epd.com
10117 Berlin www.ibu-epd.com
Germany
Author of the Life Cycle Assessment
FORCE Technology +4543250856
Park Alle 345 chme@force.dk
2605 Brøndby www.forcetechnology.com
Denmark
Owner of the Declaration
VELUX Group +4545164726
Ådalsvej 99 jakob.roerbech@velux.com
2970 Hørsholm www.velux.com
Denmark
6 Environmental Product Declaration - VELUX Group - Window operator for VELUX pivot hinged windows and KSX 100K (for retrofitting), solar powered
