ENVIRONMENTAL PRODUCT DECLARATION
as per ISO 14025 and EN 15804+A1
Owner of the Declaration Associated Weavers Europe NV
Programme holder Institut Bauen und Umwelt e.V. (IBU)
Publisher Institut Bauen und Umwelt e.V. (IBU)
Declaration number EPD-AWE-20220157-CBA1-EN
Issue date 25.05.2022
Valid to 24.05.2027
Sedna Range
Tufted broadloom carpets with a total pile weight of 800 g/m2
and a pile material of 100% regenerated polyamide 6
Associated Weavers Europe NV
www.ibu-epd.com | https://epd-online.com
Umwelt Produktdeklaration Name des Herstellers – Name des Produkts
General Information
Associated Weavers Europe NV Sedna Range
Tufted broadloom carpet
Total weight of 800 g/m2 100%
regenerated PA6 yarn
Textile polyester backing with 100%
recycled material
Programme holder Owner of the declaration
IBU – Institut Bauen und Umwelt e.V. Associated Weavers Europe NV
Hegelplatz 1 Industriepark Klein Frankrijk
10117 Berlin Weverijstraat 1
Germany 9600 Ronse
Belgium
Declaration number Declared product / declared unit
EPD-AWE-20220157-CBA1-EN Sedna Range - 1 m² tufted broadloom carpet with a
surface pile of 100% regenerated PA 6 and a polyester
Eco FusionBac backing.
This declaration is based on the product Scope:
category rules: The manufacturer declaration applies to broadloom
Floor coverings, 02/2018 carpets with Eco FusioBac, a pile material of PA 6 with
(PCR checked and approved by the SVR) 100% recycled content and a total pile weight of 800
g/m2. The products are produced in Ronse, Belgium.
Issue date
25.05.2022
The owner of the declaration shall be liable for the
Valid to underlying information and evidence; the IBU shall not
be liable with respect to manufacturer information, life
24.05.2027
cycle assessment data and evidences.
The EPD was created according to the specifications
of EN 15804+A1. In the following, the standard will be
simplified as EN 15804.
Verification
The standard EN 15804 serves as the core PCR
Independent verification of the declaration and data
according to ISO 14025:2011
Dipl. Ing. Hans Peters internally x externally
(chairman of Institut Bauen und Umwelt e.V.)
Dr. Alexander Röder Angela Schindler
(Managing Director Institut Bauen und Umwelt e.V.)) (Independent verifier)
Product
Product description/Product definition Regulation (CPR) applies. The product needs a
Tufted broadloom carpets having a surface pile of Declaration of Performance (DoP) taking into
100% regenerated polyamide 6 and an Eco FusionBac consideration EN 14041: 2018-05, Resilient, textile and
backing. The colour of the carpet is generated by laminate floor coverings - Essential characteristics, and
continuous dyeing. The total recycled content amounts the CE-marking. The DoP of the product can be found
to 52 % with a total pile weight of 800 g/m2. The on the manufacturer's technical information section.
declaration applies to a product with a total pile weight For the application and use of the product the
of 800 g/m2. respective national provisions apply.
For the placing on the market of the product in the Application
European Union/European Free Trade Association According to the use class as defined in EN 1307 the
(EU/EFTA) (with the exception of Switzerland) products can be used in all professional areas. The
Regulation (EU) No. 305/2011 Construction Product use class can be found on the technical data sheet of
the product.
2 Environmental Product Declaration Associated Weavers Europe NV (AW) – Sedna Range - Tufted Broadloom carpet with
a pile weight of 800 g/m2 and 100% recycled PA6 yarn
This product contains substances listed in the ECHA
Technical Data candidate list (16.01.2020) or other carcinogenic,
mutagenic or reprotoxic (CMR) substances in
categories 1A or 1B which are not on the candidate list
exceeding 0.1 percentage by mass: no.
Name Value Unit The products are registered in the GUT-PRODIS
Product Form broadloom carpets - Information System. The PRODIS system ensures the
Type of manufacture Tufted carpets - compliance with limitations of various chemicals and
Yarn type Polyamide 6 - Volatile Organic Compound (VOC)-emissions and a
continuous dyed ban on the use of all substances that are listed as
Coloration
surface 'Substances of Very High Concern' (SVHC) under
Primary backing Polypropylene REACH.
Secondary backing Polyester -
Total pile weight 800 g/m² Reference service life
A calculation of the reference service life according to
Total carpet weight 1552 g/m2
ISO 15686 is not possible.
The service life of textile floor coverings strongly
depends on the correct installation taking into account
Performance data of the product in accordance with
the declared use classification and the adherence to
the declaration of performance with respect to its
cleaning and maintenance instructions.
essential characteristics according to EN 14041: 2018-
A minimum service life of 10 years can be
05, Resilient, textile and laminate floor coverings -
assumed, technical service life can be considerably
Essential characteristics. Additional product properties
longer.
in accordance with EN 1307 can be found on the
Product Information System PRODIS using the
PRODIS registration number of the product (www.pro-
dis.info) or on the manufacturer's technical information
section (www.carpetyourlife.com).
Base materials/Ancillary materials
Name Value Unit
Polyamide 6 51,6 %
Polyester 6,3 %
SBR-latex 8,3 %
Polypropylene 6,4 %
Limestone 27,4 %
Additives 0,03 %
LCA: Calculation rules
Declared Unit emissions, waste water treatment, packaging material
and waste processing up to the landfill disposal of
residual waste (except radioactive waste). Benefits for
Name Value Unit generated electricity and steam due to the incineration
Declared unit 1 m2 of production waste are aggregated.
Conversion factor to 1 kg 1.55 - Biogenic carbon that is stored in renewable material
The declared unit refers to 1 m2 produced textile floor (packaging paper) is taken into account as well as the
covering. The output of module A5 'Assembly' is 1 m2 associated carbon dioxide uptake from the air from
installed textile floor covering. which this biogenic carbon comes.
A4 Transport:
System boundary Transport of the packed textile floor covering
from factory gate to the place of installation.
Type of EPD: Cradle-to-grave
A5 Installation:
System boundaries of modules A, B, C, D: Installation of the textile floor covering, processing of
Modules C3, C4 and D are indicated separately for installation waste and packaging waste up to the
three end-of-life scenarios: landfill disposal of residual waste (except radioactive
1 - landfill disposal waste), the production of the amount of carpet that
2 - municipal waste incineration occurs as installation waste including its transport to
3 - recovery in a cement plant the place of installation.
Generated electricity and steam due to the incineration
of waste are listed in the result table as exported
energy.
A1-A3 Production: Biogenic carbon that is stored in renewable materials
Energy supply and production of the basic material, in packaging paper is released as carbon dioxide
processing of secondary material, auxiliary material, emissions into the air at the end of life in module A5.
transport of the material to the manufacturing site,
3 Environmental Product Declaration Associated Weavers Europe NV (AW) – Sedna Range - Tufted Broadloom carpet with
a pile weight of 800 g/m2 and 100% recycled PA6 yarn
Preparation of the floor and auxiliary materials C3-3: Collection of the carpet waste for recovery in the
(adhesives, fixing agents, PET connectors) are beyond cement industry, waste processing (granulating),
the system boundaries and not taken into account. transport to the cement plant, emissions from the
incineration. The biogenic carbon that is stored in the
B1 Use: renewable materials of the floor covering is released
Indoor emissions during the use stage. After the first into the air as carbon dioxide emissions.
year, no product-related Volatile Organic Compound
(VOC) emissions are relevant due to known VOC C4 Disposal
decay curves of the product. C4-1: Impact from landfill disposal,
C4-2: The carpet waste leaves the system in
B2 Maintenance: module C3-2,
Cleaning of the textile floor covering for a period of 1 C4-3: The pre-processed carpet waste leaves the
year: system in module C3-3.
Vacuum cleaning – electricity supply
Wet cleaning – electricity, water consumption, D Recycling potential:
production of the cleaning agent, waste water Calculated benefits result from materials exclusive
treatment. secondary materials (net materials).
The declared values in this module have to be D-A5: Benefits for generated energy due
multiplied by the assumed service life of the floor to incineration of packaging and installation waste
covering in the building in question. (incineration plant with R1 > 0.6),
D-1: Benefits for generated energy due to landfill
B3 - B7: disposal of carpet waste at the end-of-life,
The modules are not relevant and therefore not D-2: Benefits for generated energy due to incineration
declared. of carpet waste at the end-of-life (incineration plant
with R1 > 0.6),
C1 De-construction: D-3: Benefits for saved fossil energy and saved
The floor covering is de-constructed manually and no inorganic material due to recovery of the carpet in a
additional environmental impact is caused. cement plant.
C2 Transport: Comparability
Transport of the carpet waste to a landfill, to the Basically, a comparison or an evaluation of EPD data
municipal waste incineration plant (MWI) or to the is only possible if all the data sets to be compared
waste collection facility for recycling. were created according to EN 15804 and the building
context, respectively the product-specific
C3 Waste processing: characteristics of performance, are taken into account.
C3-1: Landfill disposal needs no waste processing.
C3-2: Impact from waste incineration (plant with Background data are taken from the GaBi database
R1>0.6), generated electricity and steam are listed in 2021. Remaining data gaps are covered by the
the result table as exported energy. ecoinvent 3.7 database
LCA: Scenarios and additional technical information
The following information refer to the declared modules specific useful life can be established. Based on this
and are the basis for calculations or can be used for useful life the effects of Module B2 need to be
further calculations. calculated in order to obtain the overall environmental
impacts.
Transport to the construction site (A4) Name Value Unit
Name Value Unit Maintenance cycle (wet cleaning) 1.5 1/year
Litres of fuel (truck, EURO 0-6 Maintenance cycle (vacuum cleaning) 208 1/year
0.0036 l/100km
mix) Water consumption (wet cleaning) 0.004 m3
Transport distance 700 km Cleaning agent (wet cleaning) 0.09 kg
Capacity utilisation (including Electricity consumption 0.314 kWh
55 %
empty runs) Further information on cleaning and maintenance see
www.carpetyourlife.com
Installation in the building (A5)
Name Value Unit End of Life (C1-C4)
Material loss 0.14 kg Three different end-of-life scenarios are declared and
Polyethylene packaging waste and installation waste the results are indicated separately in module C.
are considered to be incinerated in a municipal waste Each scenario is calculated as a 100 % scenario.
incineration plant. Cardboard is going to be recycled.
Preparation of the floor and auxiliaries (adhesives, Scenario 1: 100 % landfill disposal
fixing agents, PET connectors etc.) are not taken into Scenario 2: 100 % municipal waste incineration (MWI)
account. with R1>0.6
Scenario 3: 100 % recycling in the cement industry
Maintenance (B2)
The values for cleaning refer to 1 m2 floor covering If combinations of these scenarios have to be
used in commercial areas per year. Depending on the calculated this should be done according to the
application based on ISO 10874, the technical service following scheme:
life recommended by the manufacturer and the EOL-impact = x % impact (Scenario 1)
anticipated strain on the floor by customers, the case- + y % impact (Scenario 2)
4 Environmental Product Declaration Associated Weavers Europe NV (AW) – Sedna Range - Tufted Broadloom carpet with
a pile weight of 800 g/m2 and 100% recycled PA6 yarn
+ z % impact (Scenario 3)
with x % + y % + z % = 100 %
Name Value Unit
Collected as mixed construction
1.55 kg
waste (scenario 1 and 2)
Collected separately (scenario 3) 1.55 kg
Landfilling (scenario 1) 1.55 kg
Energy recovery (scenario 2) 1.55 kg
Energy recovery (scenario 3) 1,13 kg
Recycling (scenario 3) 0.42 kg
Reuse, recovery and/or recycling potentials (D),
relevant scenario information
Recovery or recycling potentials due to the three end-
of-life scenarios (module C) are indicated separately.
Recycling in the cement industry (scenario 3)
VDZ e.V.
The organic material of the carpet is used as
secondary fuel in a cement kiln. It mainly substitutes
for lignite (65.5 %), hard coal (26.2 %) and petrol coke
(8.6 %).
The inorganic material is substantially integrated into
the cement clinker and substitutes for original material
input.
5 Environmental Product Declaration Associated Weavers Europe NV (AW) – Sedna Range - Tufted Broadloom carpet with
a pile weight of 800 g/m2 and 100% recycled PA6 yarn
LCA: Results
The LCA results refer to a product with a total pile weight of 800 g/m2. The declared result figures in module B2
have to be multiplied by the assumed service life (in years) of the floor covering in the building under
consideration. Information on non-relevant modules: Modules B3 - B7 are not relevant during the service life of
the carpet. Modules C1, C3/1, C4/2 and C4/3 cause no additional impact (see chapter "LCA: Calculation rules" in
this document). All these modules are declared and marked as 'modules not relevant/declared'. Module C2
represents the transport for scenarios 1, 2 and 3. Column D represents module D/A5. The calculations are based
on the CML characterization factors (version August 2016).
DESCRIPTION OF THE SYSTEM BOUNDARY (X = INCLUDED IN LCA; MND = MODULE NOT DECLARED;
MNR = MODULE NOT RELEVANT)
BENEFITS AND
CONSTRUCTI LOADS
PRODUCT STAGE ON PROCESS USE STAGE END OF LIFE STAGE BEYOND THE
STAGE SYSTEM
BOUNDARIES
6 Environmental Product Declaration Associated Weavers Europe NV (AW) – Sedna Range - Tufted Broadloom carpet with
a pile weight of 800 g/m2 and 100% recycled PA6 yarn
lairetam
waR
ylppus tropsnarT
gnirutcafunaM
eht
morf
tropsnarT
etis
eht
ot
etag
ylbmessA esU
ecnanetniaM
riapeR
tnemecalpeR tnemhsibrufeR
ygrene
lanoitarepO esu
retaw
lanoitarepO esu
noitcurtsnoc-eD
noitilomed tropsnarT
gnissecorp
etsaW
lasopsiD -esueR -yrevoceR -gnilcyceR laitnetop
A1 A2 A3 A4 A5 B1 B2 B3 B4 B5 B6 B7 C1 C2 C3 C4 D
X X X X X X X MNR MNR MNR MND MND MND X X X X
RESULTS OF THE LCA - ENVIRONMENTAL IMPACT according to EN 15804+A1: 1 m² floorcovering
Parameter Unit A1-A3 A4 A5 B1 B2 C2 C3/2 C3/3 C4/1 D D/1 D/2 D/3
GWP [kg CO2-Eq.] 3.34E+0 9.18E-2 5.92E-1 0.00E+0 1.71E-1 5.15E-3 2.73E+0 2.79E+0 1.05E-1 -2.35E-2 0.00E+0 -1.67E-1 -4.30E-2
-3.57E- -2.49E- -1.88E-
ODP [kg CFC11-Eq.] 9.41E-9 1.60E-178.47E-100.00E+0 2.37E-9 8.99E-197.55E-161.03E-153.58E-16 0.00E+0
16 15 16
AP [kg SO2-Eq.] 9.76E-3 3.80E-4 1.13E-3 0.00E+0 4.46E-4 2.13E-5 2.34E-3 2.41E-3 2.73E-4 -2.71E-5 0.00E+0 -1.91E-4 -1.17E-4
EP [kg (PO4)3--Eq.] 2.13E-3 9.68E-5 2.56E-4 0.00E+0 9.11E-5 5.42E-6 6.05E-4 6.21E-4 2.97E-4 -3.73E-6 0.00E+0 -2.63E-5 -1.93E-5
POCP [kg ethene-Eq.] 7.58E-4 -1.63E-4 6.56E-5 6.29E-5 4.69E-5 -9.12E-6 1.41E-4 1.19E-4 2.46E-5 -2.49E-6 0.00E+0 -1.76E-5 -1.58E-5
ADPE [kg Sb-Eq.] 2.78E-6 8.15E-9 2.55E-7 0.00E+0 6.39E-7 4.57E-10 5.04E-8 5.44E-8 2.02E-8 -4.39E-9 0.00E+0 -3.08E-8 -4.84E-9
ADPF [MJ] 5.52E+1 1.25E+0 5.20E+0 0.00E+0 2.68E+0 7.01E-2 1.27E+0 1.55E+0 1.57E+0 -3.38E-1 0.00E+0-2.41E+0-6.24E+0
GWP = Global warming potential; ODP = Depletion potential of the stratospheric ozone layer; AP = Acidification potential of land and water; EP =
Caption Eutrophication potential; POCP = Formation potential of tropospheric ozone photochemical oxidants; ADPE = Abiotic depletion potential for non-
fossil resources; ADPF = Abiotic depletion potential for fossil resources
RESULTS OF THE LCA - INDICATORS TO DESCRIBE RESOURCE USE according to EN 15804+A1: 1 m²
floorcovering
Parameter Unit A1-A3 A4 A5 B1 B2 C2 C3/2 C3/3 C4/1 D D/1 D/2 D/3
PERE [MJ] 3.94E+1 7.00E-2 3.65E+0 0.00E+0 1.15E+0 3.92E-3 1.72E-1 2.52E-1 1.18E-1 -9.19E-2 0.00E+0 -6.43E-1 -4.64E-2
PERM [MJ] 7.30E-2 0.00E+0 -7.30E-2 0.00E+0 0.00E+0 0.00E+0 0.00E+0 0.00E+0 0.00E+0 0.00E+0 0.00E+0 0.00E+0 0.00E+0
PERT [MJ] 3.95E+1 7.00E-2 3.57E+0 0.00E+0 1.15E+0 3.92E-3 1.72E-1 2.52E-1 1.18E-1 -9.19E-2 0.00E+0 -6.43E-1 -4.64E-2
PENRE [MJ] 5.30E+1 1.26E+0 5.90E+0 0.00E+0 3.64E+0 7.04E-2 8.34E+0 8.67E+0 1.62E+0 -4.13E-1 0.00E+0 -2.93E+0 -6.27E+0
PENRM [MJ] 7.21E+0 0.00E+0 -2.41E-1 0.00E+0 0.00E+0 0.00E+0 -6.97E+0 -6.97E+0 0.00E+0 0.00E+0 0.00E+0 0.00E+0 0.00E+0
PENRT [MJ] 6.02E+1 1.26E+0 5.66E+0 0.00E+0 3.64E+0 7.04E-2 1.38E+0 1.70E+0 1.62E+0 -4.13E-1 0.00E+0 -2.93E+0 -6.27E+0
SM [kg] 9.50E-1 0.00E+0 8.55E-2 0.00E+0 0.00E+0 0.00E+0 0.00E+0 0.00E+0 0.00E+0 0.00E+0 0.00E+0 0.00E+0 2.40E-1
RSF [MJ] 0.00E+0 0.00E+0 0.00E+0 0.00E+0 0.00E+0 0.00E+0 0.00E+0 0.00E+0 0.00E+0 0.00E+0 0.00E+0 0.00E+0 0.00E+0
NRSF [MJ] 0.00E+0 0.00E+0 0.00E+0 0.00E+0 0.00E+0 0.00E+0 0.00E+0 0.00E+0 0.00E+0 0.00E+0 0.00E+0 0.00E+0 0.00E+0
FW [m³] 9.63E-2 8.01E-5 9.37E-3 0.00E+0 1.77E-3 4.49E-6 7.31E-3 7.39E-3 1.50E-5 -8.98E-5 0.00E+0 -6.28E-4 -5.10E-4
PERE = Use of renewable primary energy excluding renewable primary energy resources used as raw materials; PERM = Use of
renewable primary energy resources used as raw materials; PERT = Total use of renewable primary energy resources; PENRE = Use of
non-renewable primary energy excluding non-renewable primary energy resources used as raw materials; PENRM = Use of non-
Caption
renewable primary energy resources used as raw materials; PENRT = Total use of non-renewable primary energy resources; SM = Use
of secondary material; RSF = Use of renewable secondary fuels; NRSF = Use of non-renewable secondary fuels; FW = Use of net fresh
water
RESULTS OF THE LCA – WASTE CATEGORIES AND OUTPUT FLOWS according to EN 15804+A1:
1 m² floorcovering
Parameter Unit A1-A3 A4 A5 B1 B2 C2 C3/2 C3/3 C4/1 D D/1 D/2 D/3
HWD [kg] 2.28E-3 6.32E-11 2.05E-4 0.00E+0 6.35E-10 3.55E-12 3.10E-10 3.59E-10 2.92E-10 -9.25E-11 0.00E+0 -6.54E-10-3.98E-11
NHWD [kg] 3.40E-1 1.86E-4 5.09E-2 0.00E+0 2.59E-3 1.05E-5 2.25E-1 2.25E-1 1.55E+0 -1.92E-4 0.00E+0 -1.35E-3 -1.55E-4
RWD [kg] 1.93E-3 1.52E-6 1.77E-4 0.00E+0 3.57E-4 8.51E-8 4.00E-5 6.29E-5 1.88E-5 -2.96E-5 0.00E+0 -2.07E-4 -1.03E-5
CRU [kg] 0.00E+0 0.00E+0 0.00E+0 0.00E+0 0.00E+0 0.00E+0 0.00E+0 0.00E+0 0.00E+0 0.00E+0 0.00E+0 0.00E+0 0.00E+0
MFR [kg] 6.39E-3 0.00E+0 2.45E-2 0.00E+0 0.00E+0 0.00E+0 0.00E+0 2.40E-1 0.00E+0 0.00E+0 0.00E+0 0.00E+0 0.00E+0
MER [kg] 0.00E+0 0.00E+0 0.00E+0 0.00E+0 0.00E+0 0.00E+0 0.00E+0 0.00E+0 0.00E+0 0.00E+0 0.00E+0 0.00E+0 0.00E+0
EEE [MJ] 0.00E+0 0.00E+0 4.68E-1 0.00E+0 0.00E+0 0.00E+0 4.79E+0 0.00E+0 0.00E+0 0.00E+0 0.00E+0 0.00E+0 0.00E+0
EET [MJ] 0.00E+0 0.00E+0 8.45E-1 0.00E+0 0.00E+0 0.00E+0 8.65E+0 0.00E+0 0.00E+0 0.00E+0 0.00E+0 0.00E+0 0.00E+0
HWD = Hazardous waste disposed; NHWD = Non-hazardous waste disposed; RWD = Radioactive waste disposed; CRU = Components
Caption for re-use; MFR = Materials for recycling; MER = Materials for energy recovery; EEE = Exported electrical energy; EEE = Exported
thermal energy
References
EN 1307 CML characterization factors
DIN EN 1307: 2014+A1:2016+A2:2018-05: Textile Impact assessment characterization factors, version
floor coverings - Classification 4.7, August 2016, Institute of Environmental Sciences -
'Centrum voor Milieuwetenschappen in Leiden' (CML),
EN 13501-1 Leiden, The Netherlands
DIN EN 13501-1:2019-05: Fire classification of
construction products and building elements - Part 1:
Classification using data from reaction to fire tests ECHA candidate list
Candidate List of substances of very high concern
EN 14041 (SVHCs) for authorisation, 16.01.2020, European
DIN EN 14041: 2018-05: Resilient, textile and laminate Chemicals Agency (ECHA), Helsinki, Finland
floor coverings - Essential characteristics
ecoinvent 3.7
EN 15804 ecoinvent, Zurich, Switzerland, database version 3.7,
EN 15804:2012-04+A1 2013/, Sustainability of published September 2020
construction works — Environmental Product
Declarations — Core rules for the product category of GaBi database 2021
construction products GaBi Software-System and Database for Life Cycle
Engineering, thinkstep AG, Leinfelden-Echterdingen,
EN 16810 Database release 2021-2
DIN EN 16810: 2017-08: Resilient, textile and laminate
floor coverings – Environmental product declarations – IBU 2021
Product category rules IBU (2021): General Programme Instructions for the
Preparation of EPDs at the Institut Bauen und Umwelt
ISO 10874 e.V., Version 2.0 Institut Bauen und Umwelt e.V.,
DIN EN ISO 10874: 2012+A1:2021-04: Resilient, Berlin. www.ibu-epd.de
textile and laminate floor coverings - Classification
PCR Part A
ISO 14025 Product Category Rules for Construction Products
DIN EN /ISO 14025:2011-10/, Environmental labels from the range of Environmental Product Declarations.
and declarations — Type III environmental Part A: Calculation Rules for the Life Cycle
declarations — Principles and procedures Assessment and Requirements on the Background
Report, V1.9, Berlin: Institut Bauen und Umwelt e.V.
ISO 14040 (IBU), January 2021
DIN EN ISO 14040:2006+A1:2020 Environmental
management - Life cycle assessment - Principles and PCR Part B
framework Product Category Rules for Construction Products
from the range of Environmental Product Declarations
ISO 14044 of Institut Bauen und Umwelt (IBU),
DIN EN ISO 14044:2006+A1:2018+A2:2020 Part B: Requirements on the EPD for floor coverings,
Environmental management - Life cycle assessment - V1.2, Berlin: Institut Bauen und Umwelt e.V. (IBU),
Requirements and guidelines February 2018
ISO 15686 PRODIS
ISO 15686: Buildings and constructed assets - Product Information System (PRODIS) of the
Service life planning European Carpet Industry, Gemeinschaft
ISO 15686-1: 2011-05: Part 1: General principles and umweltfreundlicher Teppichboden e.V (GUT) and
framework European Carpet and Rug Association
ISO 15686-2: 2012-05: Part 2: Service life prediction (ECRA), http://www.pro-dis.info
procedures
ISO 15686-7: 2017-04: Part 7: Performance REACH
evaluation for feedback of service life data Regulation (EC) No 1907/2006 of the European
from practice Parliament and of the Council of 18 December 2006
ISO 15686-8: 2008-06: Part 8: Reference service life concerning the Registration, Evaluation, Authorisation
and service-life estimation and Restriction of Chemicals (REACH). Last update:
27.02.2020 (Status: 27.06.2018)
Regulation (EU) No. 305/2011
Regulation No. 305/2011 Construction Products VDZ e.V.
Regulation (CPR) of the European Council and of the Association of German Cement Works, Ed.
European Parliament, April 2011 Environmental Data of the German Cement Industry
2019
7 Environmental Product Declaration Associated Weavers Europe NV (AW) – Sedna Range - Tufted Broadloom carpet with
a pile weight of 800 g/m2 and 100% recycled PA6 yarn
Publisher
Institut Bauen und Umwelt e.V. Tel +49 (0)30 3087748- 0
Hegelplatz 1 Fax +49 (0)30 3087748- 29
10117 Berlin Mail info@ibu-epd.com
Germany Web www.ibu-epd.com
Programme holder
Institut Bauen und Umwelt e.V. Tel +49 (0)30 - 3087748- 0
Hegelplatz 1 Fax +49 (0)30 – 3087748 - 29
10117 Berlin Mail info@ibu-epd.com
Germany Web www.ibu-epd.com
Author of the Life Cycle
Assessment Tel +49 (0)241 96843 410
Gemeinschaft umweltfreundlicher Fax +49 (0)241 96843 400
Teppichboden (GUT) e.V. Mail mail@gut-ev.de
Schönebergstraße 2 Web www.gut-ev.org
52068 Aachen
Germany
Owner of the Declaration
Associated Weavers Europe NV Tel +32 (0) 55 23 02 11
Weverijstraat 1 Fax -
9600 Ronse Mail info@awe.be
Belgium Web www.carpetyourlife.com
