ENVIRONMENTAL PRODUCT DECLARATION
as per ISO 14025 and EN 15804+A2
Owner of the Declaration dormakaba International Holding GmbH
Publisher Institut Bauen und Umwelt e.V. (IBU)
Programme holder Institut Bauen und Umwelt e.V. (IBU)
Declaration number EPD-DOR-20220318-CBA3-EN
Issue date 14.04.2023
Valid to 13.04.2028
ED 100/250
dormakaba
www.ibu-epd.com | https://epd-online.com
General Information
dormakaba ED 100/250
Programme holder Owner of the declaration
IBU – Institut Bauen und Umwelt e.V. dormakaba International Holding GmbH
Hegelplatz 1 DORMA Platz 1
10117 Berlin 58256 Ennepetal
Germany Germany
Declaration number Declared product / declared unit
EPD-DOR-20220318-CBA3-EN 1 piece of the product: Automatic Swing Door Operator ED 100, consisting
of the following items:
- ED 100 swing door operator
- ED slide channel set
- ED basic cover
- Product packaging
This declaration is based on the product category rules: Scope:
Drive systems for automatic doors and gates, 01.08.2021 This Environmental Product Declaration refers to a specific ED 100
(PCR checked and approved by the SVR) automaic swing door operator manufacutred by dormakaba. This EPD is
also representative for the ED 250. The production site is located in
Ennepetal (Germany). Green electricity is being used at the production
Issue date site.
14.04.2023
Data represents the year 2022.
The owner of the declaration shall be liable for the underlying information
and evidence; the IBU shall not be liable with respect to manufacturer
Valid to
information, life cycle assessment data and evidences.
13.04.2028
The EPD was created according to the specifications of EN 15804+A2. In
the following, the standard will be simplified as EN 15804.
Verification
The standard EN 15804 serves as the core PCR
Independent verification of the declaration and data according to ISO
14025:2011
internally X externally
Dipl.-Ing. Hans Peters
(Chairman of Institut Bauen und Umwelt e.V.)
Florian Pronold Dr.-Ing. Wolfram Trinius,
(Managing Director Institut Bauen und Umwelt e.V.) (Independent verifier)
1 Environmental Product Declaration - dormakaba - ED 100/250
Product
Product description/Product definition The ED 100/250 has the following technical properties:
The automatic swing door operators manufactured by
Name Value Unit
dormakaba are electromechanical swing door operators
Height 240 mm
designed for single- or double leaf doors. Depending on the
width and weight of the door leaf, the ED 100 or the ED 250 is Installation depth 152 mm
required. Both operators can be mounted with standard arm as Maximum door weight ED 100 272 kg
push-version and with slide channel as pull-version. Apart from Opening speed maximum 50 cm/s
the extended cover, an integrated door coordinator is also
Closing speed maximum 40 cm/s
available for double-leaf operators, which is also easily fitted.
Hold open time maximum 60 s
By using the dormakaba upgrade card, the functional scope
can be adapted to a variety of door situations. Supply voltage, frequency maximum 60 Hz
Power consumption 175 W
Features Class of protection 20 IP
• Flexible configuration of the functions actually required Performance data of the product with respect to its
• Inexpensive transport and easy assembly thanks to characteristics in accordance with the relevant technical
lower weights provision which can be applied are mentioned above.
• Low-noise application thanks to multi-stage gear
• Elegant design: dormakaba Contur Design with an Base materials/Ancillary materials
operator height of only 70 mm The major material composition including the packaging of the
For the use and application of the product the respective product is listed below.
national provisions at the place of use apply.
Name Value Unit
• ISO 13849-1 Steel 33 %
• DIN 18650-1
Aluminium 19 %
• DIN 18650-2
Paper 14 %
• EN 16005
• EN 60335-1 Zinc 14 %
• 2011/65/EU ROHS3 Directive Plastic 10 %
• Machinery Directive 2006/42/EC Electronics 9 %
The CE-marking takes into account the proof of conformity with
Brass 1 %
the respective harmonized standards based on the legal
provisions above. The ED100/250 includes partial articles which contain
substances listed in the Candidate List of REACH Regulation
Application 1907/2006/EC (date: 17.01.2023) exceeding 0.1 percentage by
dormakaba swing door operators are suitable for various mass: yes
applications: • Lead (Pb): 7439-92-1 (CAS-No) is used in the steel
• For single- or double- leaf swing doors alloy. The concentration of lead in the alloy does not
• Assembly on smoke or fire doors: as pull- version with exceed 0,35% (by mass).
slide channels and as push- version with standard arm The Candidate List can be found on the ECHA website
• Automation of doors with low traffic capacity (Low- address: https:echa.europa.eu/de/home.
Energy Mode) and heavily frequented doors (Full-
Reference service life
Energy Mode)
• High torque for full-automatic swing doors with radar The reference service life of the ED 100 and ED 250 amounts
detector control to 10 years and depends on the application and frequency of
• Suitable for internal and external doors use. Regular maintenance is advised to ensure the life
expectancy of 10 years. For repairs or renewals, suitable spare
parts are available. The swing door operators are tested and
certified to EN 16005, meaning they are designed to withstand
Technical Data a minium of 1.000.000 cycles.
LCA: Calculation rules
Production - Module A1-A3
Declared Unit The product stage includes:
— A1, raw material extraction, processing and mechanical
The declared unit is 1 piece of the product: ED 100/250 treatments, processing of secondary material input (e.g.
Name Value Unit recycling processes),
— A2, transport to the manufacturer,
Declared unit 1 pce.
— A3, manufacturing and assembly including provision of all
Mass reference 13.54 kg/pce
materials, products and energy, as well as waste processing up
to the end-of waste state.
System boundary
The type of EPD is: cradle to gate with options, modules C1– Construction stage - Modules A4-A5
C4, and module D (A1–A3 + C + D and additional modules: A4 The construction process stage includes:
+ A5 + B6) — A4, transport to the building site;
— A5, installation into the building; including provision of all
2 Environmental Product Declaration - dormakaba - ED 100/250
materials, products and energy, as well as waste processing up includes:
to the end-of waste state or disposal of final residues during the — D, recycling potentials, expressed as net impacts and
construction process stage. benefits.
Use stage - Module B6 Geographic Representativeness
The use stage related to the operation of the building Land or region, in which the declared product system is
includes: manufactured, used or handled at the end of the product´s
— B6, operational energy use lifespan: Global
End-of-life stage– Modules C1-C4 and D
Comparability
The end-of-life stage includes:
Basically, a comparison or an evaluation of EPD data is only
— C1, de-construction, demolition:
possible if all the data sets to be compared were created
— C2, transport to waste processing;
according to EN 15804 and the building context, respectively
— C3, waste processing for reuse, recovery and/or recycling;
the product-specific characteristics of performance, are taken
— C4, disposal; including provision and all transport, provision
into account. Background database: GaBi, SP40
of all materials, products and related energy and water use.
Module D (Benefits and loads beyond the system boundary)
LCA: Scenarios and additional technical information
Name Value Unit
Characteristic product properties of biogenic carbon
Electricity consumption ED 100 for 1 year 70.42 kWh
Information on describing the Biogenic Carbon Content at Days per year in use 365 days
factory gate
On mode per day 1.8 h
Name ValueUnit
Idle mode per day 22.2 h
kg
Biogenic carbon content in product 0.27 On mode power 22.09 W
C
Idle mode power 6.9 W
Biogenic carbon content in accompanying kg
0.41
packaging C End of life (C1-C4)
C1: The product dismantling from the building is done manually
Additional technical information for the declared modules. without environmental burden.
Name Value Unit
Transport from the gate to the site (A4) Collected separately waste type 12.43 kg
Name Value Unit Recycling 8.18 kg
Litres of fuel (per 1 kg) 0.00276 l/100km Energy recovery 1.89 kg
Capacity utilisation (including empty runs) 55 % Landfilling 2.36 kg
Transport distance via medium truck 100 km Transport to waste management 50 km
The product is transported via truck. The product is stored in The product is disassembled in a recycling process.
the dormakaba logistic center in Germany. Material recycling is then assumed for the metals and
electronics. The plastic components are assumed to be
incinerated with energy recovery. Electromechanics and minor
Installation into the building (A5)
proportions of residues arising from the recycling process are
Name Value Unit
landfilled.
Waste packaging (paper and plastic) 1,11 kg Region for the End of Life is: Global.
Reuse, recovery and/or recycling potentials (D), relevant
Reference service life
scenario information
Name Value Unit
Name Value Unit
Life Span according to the manufacturer 10 a
Recycling 100 %
Operational energy use (B6)
Collection rate is 100%.
The use stage is declared for 10 years
3 Environmental Product Declaration - dormakaba - ED 100/250
LCA: Results
DESCRIPTION OF THE SYSTEM BOUNDARY (X = INCLUDED IN LCA; MND = MODULE OR INDICATOR NOT DECLARED; MNR
= MODULE NOT RELEVANT)
Benefits and
Construction loads beyond
Product stage Use stage End of life stage
process stage the system
boundaries
la ire ta m w a Ry lp p u s tro p s n a rT g n iru tc a fu n a M e h t m o rf tro p s n a rTe tis e h t o t e ta g y lb m e s s A e s U e c n a n e tn ia M ria p e R tn e m e c a lp e R tn e m h s ib ru fe R y g re n e la n o ita re p Oe s u re ta w la n o ita re p Oe s u n o itc u rts n o c -e Dn o itilo m e d tro p s n a rT g n is s e c o rp e ts a W la s o p s iD -e s u e R-y re v o c e R-g n ilc y c e Rla itn e to p
A1 A2 A3 A4 A5 B1 B2 B3 B4 B5 B6 B7 C1 C2 C3 C4 D
X X X X X MND MND MNR MNR MNR X MND X X X X X
RESULTS OF THE LCA - ENVIRONMENTAL IMPACT according to EN 15804+A2: 1 piece ED 100_250
Parameter Unit A1-A3 A4 A5 B6 C1 C2 C3 C4 D
GWP-total kg CO 2 eq 5.01E+01 1.18E-01 1.57E+00 2.85E+02 0 6.2E-02 6.22E+00 4.2E-02 -1.39E+01
GWP-fossil kg CO 2 eq 5.27E+01 1.13E-01 3.9E-02 2.83E+02 0 5.9E-02 4.89E+00 4.2E-02 -1.38E+01
GWP-biogenic kg CO 2 eq -2.72E+00 5E-03 1.53E+00 9.45E-01 0 3E-03 1.33E+00 1.43E-04 -3.6E-02
GWP-luluc kg CO 2 eq 6.7E-02 2.69E-06 2.58E-05 4.11E-01 0 1.4E-06 2.88E-04 1.21E-04 -7E-03
ODP kg CFC11 eq 4.49E-09 1.2E-17 2.83E-16 6.24E-12 0 6.22E-18 2.62E-15 1.55E-16 -2.62E-11
AP mol H+ eq 2.14E-01 1.13E-04 4.39E-04 6.26E-01 0 5.89E-05 1E-03 3.01E-04 -5.3E-02
EP-freshwater kg P eq 2.04E-04 2.42E-08 5.53E-08 7.57E-04 0 1.26E-08 4.16E-07 7.2E-08 -2.37E-05
EP-marine kg N eq 3.8E-02 3.61E-05 1.59E-04 1.39E-01 0 1.88E-05 2.58E-04 7.74E-05 -7E-03
EP-terrestrial mol N eq 4E-01 4.01E-04 2E-03 1.46E+00 0 2.09E-04 5E-03 8.5E-04 -7.9E-02
kg NMVOC
POCP 1.19E-01 1.02E-04 4.2E-04 3.81E-01 0 5.3E-05 7.12E-04 2.34E-04 -2.6E-02
eq
ADPE kg Sb eq 1.12E-02 3.4E-09 4.46E-09 8.21E-05 0 1.77E-09 3.63E-08 3.76E-09 -3E-03
ADPF MJ 8.17E+02 1.61E+00 4.95E-01 4.98E+03 0 8.35E-01 2.55E+00 5.5E-01 -1.9E+02
m3 world eq
WDP 9.42E+00 2.22E-04 1.94E-01 6.18E+01 0 1.15E-04 6.37E-01 4E-03 -1.88E+00
deprived
GWP = Global warming potential; ODP = Depletion potential of the stratospheric ozone layer; AP = Acidification potential of land and water; EP =
Eutrophication potential; POCP = Formation potential of tropospheric ozone photochemical oxidants; ADPE = Abiotic depletion potential for non-fossil
resources; ADPF = Abiotic depletion potential for fossil resources; WDP = Water (user) deprivation potential)
RESULTS OF THE LCA - INDICATORS TO DESCRIBE RESOURCE USE according to EN 15804+A2: 1 piece ED 100_250
Parameter Unit A1-A3 A4 A5 B6 C1 C2 C3 C4 D
PERE MJ 1.92E+02 5E-03 1.34E+01 2.21E+03 0 3E-03 9.52E+00 7.2E-02 -4.87E+01
PERM MJ 2.22E+01 0 -1.33E+01 0 0 0 -8.88E+00 0 0
PERT MJ 2.14E+02 5E-03 9E-02 2.21E+03 0 3E-03 6.41E-01 7.2E-02 -4.87E+01
PENRE MJ 7.36E+02 1.61E+00 4.95E-01 4.98E+03 0 8.36E-01 8.33E+01 5.5E-01 -1.9E+02
PENRM MJ 8.08E+01 0 0 0 0 0 -8.08E+01 0 0
PENRT MJ 8.17E+02 1.61E+00 4.95E-01 4.98E+03 0 8.36E-01 2.55E+00 5.5E-01 -1.9E+02
SM kg 5.66E+00 0 0 0 0 0 0 0 0
RSF MJ 0 0 0 0 0 0 0 0 0
NRSF MJ 0 0 0 0 0 0 0 0 0
FW m3 3.25E-01 9.08E-06 5E-03 2.55E+00 0 4.72E-06 1.5E-02 1.39E-04 -9.5E-02
PERE = Use of renewable primary energy excluding renewable primary energy resources used as raw materials; PERM = Use of renewable primary
energy resources used as raw materials; PERT = Total use of renewable primary energy resources; PENRE = Use of non-renewable primary energy
excluding non-renewable primary energy resources used as raw materials; PENRM = Use of non-renewable primary energy resources used as raw
materials; PENRT = Total use of non-renewable primary energy resources; SM = Use of secondary material; RSF = Use of renewable secondary fuels;
NRSF = Use of non-renewable secondary fuels; FW = Use of net fresh water
RESULTS OF THE LCA – WASTE CATEGORIES AND OUTPUT FLOWS according to EN 15804+A2:
1 piece ED 100_250
Parameter Unit A1-A3 A4 A5 B6 C1 C2 C3 C4 D
HWD kg 3.63E-05 1.56E-10 7.3E-10 2.06E-06 0 8.11E-11 8.81E-09 8.39E-09 -3.9E-06
NHWD kg 3.33E+00 1.64E-04 4.9E-02 3.54E+00 0 8.55E-05 5.16E-01 2.77E+00 -6.13E-01
RWD kg 2.8E-02 1.73E-06 2.6E-05 7.56E-01 0 8.97E-07 1E-04 6.26E-06 -1.3E-02
CRU kg 0 0 0 0 0 0 0 0 0
MFR kg 0 0 0 0 0 0 6.55E+00 0 0
MER kg 0 0 0 0 0 0 0 0 0
EEE MJ 0 0 2.37E+00 0 0 0 1.11E+01 0 0
EET MJ 0 0 4.3E+00 0 0 0 2.45E+01 0 0
4 Environmental Product Declaration - dormakaba - ED 100/250
HWD = Hazardous waste disposed; NHWD = Non-hazardous waste disposed; RWD = Radioactive waste disposed; CRU = Components for re-use;
MFR = Materials for recycling; MER = Materials for energy recovery; EEE = Exported electrical energy; EET = Exported thermal energy
RESULTS OF THE LCA – additional impact categories according to EN 15804+A2-optional:
1 piece ED 100_250
Parameter Unit A1-A3 A4 A5 B6 C1 C2 C3 C4 D
Disease
PM 2.07E-06 5.96E-10 2.43E-09 5.25E-06 0 3.1E-10 1.2E-08 3.72E-09 -6.78E-07
incidence
IR kBq U235 eq 3.34E+00 2.46E-04 4E-03 1.24E+02 0 1.28E-04 1E-02 6.44E-04 -2.1E+00
ETP-fw CTUe 3.71E+02 1.14E+00 2.35E-01 2.13E+03 0 5.92E-01 9.74E-01 3.14E-01 -6.43E+01
HTP-c CTUh 2.96E-08 2.14E-11 1.24E-11 5.89E-08 0 1.11E-11 8.17E-11 4.66E-11 2.28E-08
HTP-nc CTUh 1.55E-06 9.15E-10 5.38E-10 2.17E-06 0 4.76E-10 7.72E-09 5.13E-09 2.7E-06
SQP SQP 4.67E+02 4E-03 1.31E-01 1.59E+03 0 2E-03 7.57E-01 1.15E-01 -1.51E+01
PM = Potential incidence of disease due to PM emissions; IR = Potential Human exposure efficiency relative to U235; ETP-fw = Potential comparative
Toxic Unit for ecosystems; HTP-c = Potential comparative Toxic Unit for humans (cancerogenic); HTP-nc = Potential comparative Toxic Unit for humans
(not cancerogenic); SQP = Potential soil quality index
Disclaimer 1 – for the indicator “Potential Human exposure efficiency relative to U235”. This impact category deals mainly with the
eventual impact of low-dose ionizing radiation on human health of the nuclear fuel cycle. It does not consider effects due to possible
nuclear accidents, occupational exposure or radioactive waste disposal in underground facilities. Potential ionizing radiation from the
soil, radon and from some construction materials is also not measured by this indicator.
Disclaimer 2 – for the indicators “abiotic depletion potential for non-fossil resources”, “abiotic depletion potential for fossil resources”,
“water (user) deprivation potential, deprivation-weighted water consumption”, “potential comparative toxic unit for ecosystems”,
“potential comparative toxic unit for humans – cancerogenic”, “Potential comparative toxic unit for humans - not cancerogenic”,
“potential soil quality index”. The results of this environmental impact indicator shall be used with care as the uncertainties on these
results are high as there is limited experience with the indicator.
This EPD was created using a software tool.
References
ISO 14025
DIN EN ISO 14025:2011-10, Environmental labels and IBU 2021
declarations — Type III environmental declarations — General Instructions for the EPD programme of Institut Bauen
Principles and procedures und Umwelt e.V. Version 2.0, Berlin: Institut Bauen und Umwelt
e.V., 2021. www.ibu-epd.com
EN 15804
EN 15804+A2:2019+AC:2021, Sustainability of construction GaBi
works — Environmental Product Declarations — Core rules for Sphera Solutions GmbH Gabi Software System and Database
the product category ofconstruction products for Life Cycle Engineering 1992-2020 Version 10.0.0.71
University of Stuttgart Leinfelden-Echterdingen
EN 18650
EN 18650-1:2010, Powered pedestrian doors - Part 1: Product GaBi ts documentation
requirements and test methods GaBi life cycle inventory data documentation
(https://www.gabisoftware.com/support/gabi/gabidatabase-
EN 18650 2020-lci-documentation/)
EN 18650-2:2010, Powered pedestrian doors - Part 2: Safety at
powered pedestrian doors LCA-tool dormakaba
LCA tool, version ENS (drive system) Tool No.: IBU-DOR-
EN 16005 202108-LT1-EN Developed by Sphera Solutions GmbH
EN 16005: 2013-01, Power operated pedestrian doorsets -
Safety in use - Requirements and test methods PCR Part A
PCR – Part A: Calculation Rules for the Life Cycle Assessment
EN 60335 and Requirements on the Project Re-port according to EN
EN 60335-1, -2-103:2020-08, Household and similar electrical 15804+A2:2019, Version 1.0, Institut Bauen und Umwelt e.V.,
appliances - Safety - Part 1: General requirements www.ibu-epd.com
EN 61000 PCR Part B
EN 61000-1-2:2017-07, Electromagnetic compatibility (EMC) - PCR – Part B: Requirements for the EPD for Drive systems for
Part 1-2: General - Methodology for the achievement of automatic doors and gates, version 08/2021, Institut Bauen und
functional safety of electrical and electronic systems including Umwelt e.V., www.ibu-epd-com.
equipment with regard to electromagnetic phenomena
REACH
EN ISO 13849 Registration, Evaluation, Authorisation and Restriction of
EN ISO 13849-1:2021-08, Safety of machinery - Safety-related Chemicals (REACH), Regulation (EC) No 1907/2006
parts of control systems - Part 1: General principles for design
2011/65/EU ROHS3 Directive
Machinery Directive Directive 2011/65/EU of the European Parliament and of the
Directive 2006/42/EC of the European Parliament and of the Council of 8 June 2011 on the restriction of the use of certain
Council on machinery, and amending Directive 95/16/EC hazardous substances in electrical and electronic equipment
5 Environmental Product Declaration - dormakaba - ED 100/250
European Chemicals Agency (ECHA)
https:echa.europa.eu/de/home
6 Environmental Product Declaration - dormakaba - ED 100/250
Publisher
Institut Bauen und Umwelt e.V. +49 (0)30 3087748- 0
Hegelplatz 1 info@ibu-epd.com
10117 Berlin www.ibu-epd.com
Germany
Programme holder
Institut Bauen und Umwelt e.V. +49 (0)30 3087748- 0
Hegelplatz 1 info@ibu-epd.com
10117 Berlin www.ibu-epd.com
Germany
Author of the Life Cycle Assessment
dormakaba International Holding GmbH +49 2333 793-0
DORMA Platz 1 info.de@dormakaba.com
58256 Ennepetal www.dormakaba.com
Germany
Owner of the Declaration
dormakaba International Holding GmbH +49 2333 793-0
DORMA Platz 1 info.de@dormakaba.com
58256 Ennepetal www.dormakaba.com
Germany
7 Environmental Product Declaration - dormakaba - ED 100/250
