ENVIRONMENTAL PRODUCT DECLARATION
as per ISO 14025 and EN 15804+A2
Owner of the Declaration Kingspan Insulation B.V.
Programme holder Institut Bauen und Umwelt e.V. (IBU)
Publisher Institut Bauen und Umwelt e.V. (IBU)
Declaration number EPD-KSI-20210047-CBA1-EN
Issue date 24.03.2021
Valid to 23.03.2026
Kooltherm® K15
Kingspan Insulation B.V.
www.ibu-epd.com | https://epd-online.com
Umwelt Produktdeklaration Name des Herstellers – Name des Produkts
General Information
Kingspan Insulation B.V. Kooltherm® K15
Programme holder Owner of the declaration
IBU – Institut Bauen und Umwelt e.V. Kingspan Insulation B.V.
Panoramastr. 1 Lingewei 8
10178 Berlin 4004 LL Tiel
Germany The Netherlands
Declaration number Declared product / declared unit
EPD-KSI-20210047-CBA1-EN Kooltherm® K15 Rainscreen Board, 1 m², 100 mm
thickness, R = 5,0 m²·K/W
D
This declaration is based on the product Scope:
category rules: The insulation material Kooltherm is produced by
Insulating materials made of foam plastics, 06.2017 Kingspan Insulation B.V. at the manufacturing facility in
(PCR checked and approved by the SVR) Tiel, the Netherlands. Aluminum multilayer facing is
autohesively bonded to the insulation core during
manufacture.
Issue date
24.03.2021
In order to enable the user of the EPD to calculate the
LCA results for different thicknesses, the EPD contains
Valid to
the respective calculation rules.
23.03.2026
The owner of the declaration shall be liable for the
underlying information and evidence; the IBU shall not
be liable with respect to manufacturer information, life
cycle assessment data and evidences.
The EPD was created according to the specifications
of EN 15804+A2. In the following, the standard will be
simplified as EN 15804.
Verification
The standard EN 15804 serves as the core PCR
Independent verification of the declaration and data
according to ISO 14025:2010
Dipl. Ing. Hans Peters internally x externally
(chairman of Institut Bauen und Umwelt e.V.)
Dr. Alexander Röder Dipl. Natw. ETH Sascha Iqbal
(Managing Director Institut Bauen und Umwelt e.V.)) (Independent verifier)
Product
Product description/Product definition Application
The Kooltherm® K15 Rainscreen board is a resole rigid Due to the high insulation value and water-resistant
foam insulation material with a fiber-free core faced layer, the Kooltherm® K15 Rainscreen facade board is
one side with black composite aluminum foil and ideal for use as insulation in curtain walls. The board is
micro-perforated blank aluminum foil on the other side. supplied with a black coating, making it perfect to work
The product is available in variable thicknesses from with a facade system with open joints.
20 mm up to 200 mm. This EPD covers one of the
most commonly sold thickness of 100 mm with an R - Technical Data
D
value of 5,0 m² K/W.
For the placing on the market of the product in the
European Union/European Free Trade Association Constructional data
(EU/EFTA) (with the exception of Switzerland) Name Value Unit
Regulation (EU) No. 305/2011 CPR applies. The Compressive strength acc. to EN 826 ≥ 100 kPa
product needs a declaration of performance taking into Tensile strength perpendicular to faces
≥ 80 kPa
consideration EN 13166:2012+A2:2016 - Thermal (σmt) acc. to EN 826
insulation products for buildings - Factory made Thermal conductivity λd acc. to /EN
0.021 W/(mK)
phenolic foam (PF) products - Specification and the 13166/ for d = 20 – 44 mm
CE-marking. For the application and use the respective Thermal conductivity λd acc. to /EN
0.020 W/(mK)
national provisions apply. 13166/ for d = 45 – 120 mm
2 Environmental Product Declaration Kingspan Insulation B.V. – Kooltherm® K15
Thermal conductivity λd acc. to /EN exempt from the requirements of Article 57 and 59(1)
0.021 W/(mK)
13166/ for d = 121 - 159 mm of REACH Regulation (EC) No 1907/2006. These
products are not classified as “hazardous products”
according to any current legislation, and can hence be
Technical parameters not included are modulus of declared as follows:
elasticity as well as sound absorption (not relevant for - This article contains substances listed in the
this application) and creep (not placed under candidate list (date: 19.01.2021) exceeding 0.1
permanent load). The water absorption/moisture percentage by mass: no.
characteristics are not applicable for the product - This article contains other carcinogenic, mutagenic,
application. reprotoxic
(CMR) substances in categories 1A or 1B which are
Performance data of the product in accordance with not on the candidate list, exceeding 0.1 percentage by
the declaration of performance with respect to its mass: no.
essential characteristics according to EN - Biocide products were added to this construction
13166:2012+A2:2016 - Thermal insulation products for product or it has been treated with biocide products
buildings - Factory made phenolic foam (PF) products - (this then concerns a treated product as defined by the
Specification. (EU) Biocide Products Regulation No. 528/2012
(BPR): no.”
Base materials/Ancillary materials
The main materials are phenolic (PF) resin (between The chemical functional group of the additives used in
70-80%) with added catalyst and additives (between the resin is that of non-ionic surfactants.
15-20%). Phenolic rigid foam onto a facing material
(between 5-10%) is formed by the chemical reaction of
these materials and adding a blowing agent with no Reference service life
ozone depletion potential (ca. 5%). The reference service life is not to be declared in this
EPD as it does not cover the use stage.
In the current REACH regulations, phenolic foam
insulation products are considered “articles” and are
LCA: Calculation rules
Declared Unit - A5 installation in the building including provision of all
The declared unit (1m²) and conversion factors are materials, products and energy, as well as waste
listed in the table below. processing up to the end-of-waste state or disposal of
final residues during the construction process stage.
Declared unit
Name Value Unit The end-of-life stage is a mandatory information
Declared unit 1 m2 module and it covers:
Gross density 35 kg/m3 - C1 de-construction, demolition;
conversion factor [Mass/Declared - C2 transport to waste processing;
3.5 -
Unit] ( in kg/m² ) - C3 waste processing for reuse, recovery and/or
Grammage 3.5 kg/m2 recycling;
Layer thickness 0.1 m - C4 disposal (not applicable for this EPD) including
provision and all transport, provision of all materials,
products and related energy and water use.
System boundary Environmental burden of the incineration (R1 > 60 %)
Type of EPD: according to EN 15804: cradle to gate of the product at the end of life stage are assigned to
with options, modules C1–C4, and module D (A1–A3, the product system (C3); resulting potential credits for
C, D and additional modules: A4,A5). thermal and electrical energy from energy substitution
are declared in module D.
According to PCR Part A:
1a) declaration of one specific product from one plant Renewable electricity sources for manufacturing
of one manufacturer. All electricity used during production comes from
The product stage is a mandatory information module renewable sources.
and it covers: By generating energy one-site with solar panels and
- A1, raw material extraction and processing, with procured energy from fully certified renewable
processing of secondary material input (e.g. recycling sources. Following the global Net Zero Energy strategy
processes) from Kingspan Group plc.
- A2, transport to the manufacturer
- A3, manufacturing,
Comparability
including the provision of all materials, products and Basically, a comparison or an evaluation of EPD data
energy, packaging processing and its transport, as is only possible if all the data sets to be compared
well as waste processing up to the end-of waste state were created according to EN 15804 and the building
or disposal of final residues during the product stage. context, respectively the product-specific
The construction process stage includes: characteristics of performance, are taken into account.
- A4 transport to the building site;
Factors for different thicknesses
3 Environmental Product Declaration Kingspan Insulation B.V. – Kooltherm® K15
The LCA results for the insulation material declared in can be used for the calculation. For modules A1-A3,
this EPD refer to a product with a thickness of 100 mm. C3 and D the LCA results in chapter 5 have to be
To enable the used of EPD to calculate the results for multiplied with these factors.
different thicknesses the factors in the following table
Background data from GaBi software-system version 9
with Service Packs 39 GaBi ts is used.
LCA: Scenarios and additional technical information
Characteristic product properties
Information on biogenic Carbon Reuse, recovery and/or recycling potentials (D),
The total mass of biogenic carbon containing relevant scenario information
materials is less than 5% of the total mass of the Waste incineration with energy recuperation is
product and accompanying packaging. assumed as end-of-life scenario.
Technical information
The following technical information is a basis for the
declared modules or can be used for developing
specific scenarios in the context of a building
assessment.
Transport to the building site (A4)
Name Value Unit
Litres of fuel 103 l/100km
Transport distance 100 km
Gross density of products transported 35 kg/m3
Installation into the building (A5)
Name Value Unit
Output substances following waste
0.08 kg
treatment on site
Within A1-A3 the following packaging of the final
product is included:
Polyethylene cover and wrap: 0.06 kg/m2.
Others (mainly Expanded Polystyrene skid): 0.02
kg/m2.
The recycling of the packaging is considered in A5.
End of life (C1-C4)
The assumptions for C1 are: diesel driven excavator
(100 kW; 0.02 litre fuel per ton excavated material).
The assumptions for C2 are: Truck Euro 6, diesel
driven, 26-28 t gross weight, assumed distance 50
km.
Name Value Unit
Collected as mixed construction waste 35 kg
Energy recovery 35 kg
R1-value of waste incineration plant >60 %
4 Environmental Product Declaration Kingspan Insulation B.V. – Kooltherm® K15
LCA: Results
Disclaimer:
EP-freshwater: This indicator has been calculated as “kg P eq” as required in the characterization model
(EUTREND model, Struijs et al., 2009b, as implemented in ReCiPe;
http://eplca.jrc.ec.europa.eu/LCDN/developerEF.xhtml)
Disclaimer:
EP-freshwater: This indicator has been calculated as “kg P eq” as required in the characterization model
(EUTREND model, Struijs et al., 2009b, as implemented in ReCiPe;
http://eplca.jrc.ec.europa.eu/LCDN/developerEF.xhtml).
DESCRIPTION OF THE SYSTEM BOUNDARY (X = INCLUDED IN LCA; ND = MODULE OR INDICATOR NOT
DECLARED; MNR = MODULE NOT RELEVANT)
BENEFITS AND
CONSTRUCTI LOADS
PRODUCT STAGE ON PROCESS USE STAGE END OF LIFE STAGE BEYOND THE
STAGE SYSTEM
BOUNDARIES
5 Environmental Product Declaration Kingspan Insulation B.V. – Kooltherm® K15
lairetam
waR
ylppus tropsnarT
gnirutcafunaM
eht
morf
tropsnarT
etis
eht
ot
etag
ylbmessA esU
ecnanetniaM
riapeR
tnemecalpeR tnemhsibrufeR
ygrene
lanoitarepO esu
retaw
lanoitarepO esu
noitcurtsnoc-eD
noitilomed tropsnarT
gnissecorp
etsaW
lasopsiD -esueR -yrevoceR -gnilcyceR laitnetop
A1 A2 A3 A4 A5 B1 B2 B3 B4 B5 B6 B7 C1 C2 C3 C4 D
X X X X X ND ND MNR MNR MNR ND ND X X X X X
RESULTS OF THE LCA - ENVIRONMENTAL IMPACT according to EN 15804+A2: 1 m2 100 mm K15
Core Indicator Unit A1-A3 A4 A5 C1 C2 C3 C4 D
GWP-total [kg CO2-Eq.] 9.10E+0 2.97E-2 2.00E-1 2.24E-3 1.48E-2 7.73E+0 0.00E+0 -3.33E+0
GWP-fossil [kg CO2-Eq.] 9.05E+0 2.94E-2 2.00E-1 2.24E-3 1.47E-2 7.73E+0 0.00E+0 -3.32E+0
GWP-biogenic [kg CO2-Eq.] -1.99E-2 -1.79E-4 -3.63E-6 -1.58E-7 -8.94E-5 3.47E-4 0.00E+0 -6.44E-3
GWP-luluc [kg CO2-Eq.] 7.06E-2 4.49E-4 7.20E-6 7.59E-8 2.25E-4 7.47E-5 0.00E+0 -2.26E-3
ODP [kg CFC11-Eq.] 1.20E-8 3.57E-18 5.97E-17 2.15E-19 1.79E-18 9.26E-16 0.00E+0 -3.40E-14
AP [mol H+-Eq.] 2.86E-2 3.47E-5 2.76E-5 1.07E-5 1.74E-5 4.61E-3 0.00E+0 -6.28E-3
EP-freshwater [kg P-Eq.] 1.98E-5 1.42E-7 1.05E-8 3.98E-10 7.09E-8 1.58E-7 0.00E+0 -4.37E-6
EP-marine [kg N-Eq.] 6.06E-3 1.07E-5 7.28E-6 4.97E-6 5.35E-6 2.21E-3 0.00E+0 -1.44E-3
EP-terrestrial [mol N-Eq.] 6.28E-2 1.25E-4 1.20E-4 5.44E-5 6.27E-5 2.55E-2 0.00E+0 -1.55E-2
POCP [kg NMVOC-Eq.] 2.45E-2 2.79E-5 2.09E-5 1.41E-5 1.40E-5 5.69E-3 0.00E+0 -4.14E-3
ADPE [kg Sb-Eq.] 6.47E-6 2.05E-9 8.60E-10 5.89E-11 1.02E-9 1.58E-8 0.00E+0 -5.19E-7
ADPF [MJ] 2.15E+2 3.92E-1 7.91E-2 3.03E-2 1.96E-1 2.09E+0 0.00E+0 -5.75E+1
[m³ world-Eq
WDP 1.34E+0 6.34E-4 2.08E-2 3.91E-6 3.17E-4 7.58E-1 0.00E+0 -3.09E-1
deprived]
GWP = Global warming potential; ODP = Depletion potential of the stratospheric ozone layer; AP = Acidification potential of land and water; EP =
Caption Eutrophication potential; POCP = Formation potential of tropospheric ozone photochemical oxidants; ADPE = Abiotic depletion potential for non-
fossil resources; ADPF = Abiotic depletion potential for fossil resources; WDP = Water (user) deprivation potential
RESULTS OF THE LCA - INDICATORS TO DESCRIBE RESOURCE USE according to EN 15804+A2: 1 m2
100 mm K15
Indicator Unit A1-A3 A4 A5 C1 C2 C3 C4 D
PERE [MJ] 3.98E+1 2.27E-2 1.53E-2 8.92E-5 1.14E-2 2.78E-1 0.00E+0 -1.17E+1
PERM [MJ] 0.00E+0 0.00E+0 0.00E+0 0.00E+0 0.00E+0 0.00E+0 0.00E+0 0.00E+0
PERT [MJ] 3.98E+1 2.27E-2 1.53E-2 8.92E-5 1.14E-2 2.78E-1 0.00E+0 -1.17E+1
PENRE [MJ] 1.19E+2 3.92E-1 7.92E-2 3.04E-2 1.96E-1 9.78E+1 0.00E+0 -5.75E+1
PENRM [MJ] 9.58E+1 0.00E+0 0.00E+0 0.00E+0 0.00E+0 -9.58E+1 0.00E+0 0.00E+0
PENRT [MJ] 2.14E+2 3.92E-1 7.92E-2 3.04E-2 1.96E-1 2.09E+0 0.00E+0 -5.75E+1
SM [kg] 0.00E+0 0.00E+0 0.00E+0 0.00E+0 0.00E+0 0.00E+0 0.00E+0 0.00E+0
RSF [MJ] 0.00E+0 0.00E+0 0.00E+0 0.00E+0 0.00E+0 0.00E+0 0.00E+0 0.00E+0
NRSF [MJ] 0.00E+0 0.00E+0 0.00E+0 0.00E+0 0.00E+0 0.00E+0 0.00E+0 0.00E+0
FW [m³] 7.31E-2 3.85E-5 4.94E-4 1.65E-7 1.92E-5 1.79E-2 0.00E+0 -1.37E-2
PERE = Use of renewable primary energy excluding renewable primary energy resources used as raw materials; PERM = Use of
renewable primary energy resources used as raw materials; PERT = Total use of renewable primary energy resources; PENRE = Use of
non-renewable primary energy excluding non-renewable primary energy resources used as raw materials; PENRM = Use of non-
Caption
renewable primary energy resources used as raw materials; PENRT = Total use of non-renewable primary energy resources; SM = Use
of secondary material; RSF = Use of renewable secondary fuels; NRSF = Use of non-renewable secondary fuels; FW = Use of net fresh
water
RESULTS OF THE LCA – WASTE CATEGORIES AND OUTPUT FLOWS according to EN 15804+A2:
1 m2 100 mm K15
Indicator Unit A1-A3 A4 A5 C1 C2 C3 C4 D
HWD [kg] 8.09E-5 2.19E-8 3.71E-10 3.22E-12 1.10E-8 1.33E-9 0.00E+0 -2.37E-8
NHWD [kg] 7.22E-1 3.19E-5 1.93E-2 1.81E-7 1.59E-5 3.88E-2 0.00E+0 -2.49E-2
RWD [kg] 4.01E-3 5.32E-7 3.64E-6 3.49E-8 2.66E-7 9.39E-5 0.00E+0 -4.65E-3
CRU [kg] 0.00E+0 0.00E+0 0.00E+0 0.00E+0 0.00E+0 0.00E+0 0.00E+0 0.00E+0
MFR [kg] 0.00E+0 0.00E+0 0.00E+0 0.00E+0 0.00E+0 0.00E+0 0.00E+0 0.00E+0
MER [kg] 0.00E+0 0.00E+0 7.99E-2 0.00E+0 0.00E+0 3.50E+0 0.00E+0 0.00E+0
EEE [MJ] 0.00E+0 0.00E+0 4.43E-1 0.00E+0 0.00E+0 1.34E+1 0.00E+0 0.00E+0
EET [MJ] 0.00E+0 0.00E+0 7.98E-2 0.00E+0 0.00E+0 2.39E+1 0.00E+0 0.00E+0
HWD = Hazardous waste disposed; NHWD = Non-hazardous waste disposed; RWD = Radioactive waste disposed; CRU = Components
Caption for re-use; MFR = Materials for recycling; MER = Materials for energy recovery; EEE = Exported electrical energy; EEE = Exported
thermal energy
RESULTS OF THE LCA – additional impact categories according to EN 15804+A2-optional:
1 m2 100 mm K15
Indicator Unit A1-A3 A4 A5 C1 C2 C3 C4 D
[Disease
PM ND ND ND ND ND ND ND ND
Incidence]
[kBq U235-
IR ND ND ND ND ND ND ND ND
Eq.]
ETP-fw [CTUe] ND ND ND ND ND ND ND ND
HTP-c [CTUh] ND ND ND ND ND ND ND ND
HTP-nc [CTUh] ND ND ND ND ND ND ND ND
SQP [-] ND ND ND ND ND ND ND ND
PM = Potential incidence of disease due to PM emissions; IR = Potential Human exposure efficiency relative to U235; ETP-fw = Potential
Caption comparative Toxic Unit for ecosystems; HTP-c = Potential comparative Toxic Unit for humans (cancerogenic); HTP-nc = Potential
comparative Toxic Unit for humans (not cancerogenic); SQP = Potential soil quality index
Disclaimer 1 – for the indicator IR
This impact category deals mainly with the eventual impact of low dose ionizing radiation on human health of the
nuclear fuel cycle. It does not consider effects due to possible nuclear accidents, occupational exposure nor due
to radioactive waste disposal in underground facilities. Potential ionizing radiation from the soil, from radon and
from some construction materials is also not measured by this indicator.
Disclaimer 2 – for the indicators ADPE, ADPF, WDP, ETP-fw, HTP-c, HTP-nc, SQP
The results of this environmental impact indicator shall be used with care as the uncertainties on these results are
high or as there is limited experienced with the indicator.
References
BPR ISO 14025
The Biocidal Products Regulation (BPR, Regulation EN ISO 14025:2011-10 - Environmental labels and
(EU) 528/2012) concerns the placing on the market declarations — Type III environmental declarations —
and use of biocidal products, which are used to protect Principles and procedures
humans, animals, materials or articles against harmful
organisms like pests or bacteria, by the action of the GaBi ts
active substances contained in the biocidal product thinkstep AG: Leinfelden-Echterdingen GaBi Software-
System and Database for Life Cycle Engineering 1992-
CPR 2019
REGULATION (EU) no. 305/2011 of the European
Parliament and of the Council of 9 March 2011 laying LCA-tool
down harmonised condition for the marketing of Kingspan LCA tool, version 1.0. IBU-KSI-202001-LT1-
construction products and repealing Council Directive EN.
89/106/EC Developed by Sphera Solutions GmbH (formely
Thinkstep GmbH)
EN 13166
EN1316:2012+A2:2016: Thermal insulation produts for PCR Version 1.7, Part A
buildings. Factory made phenolic foam (PF) products. Institut Bauen und Umwelt e.V., Berlin (pub.): Product
Specification Category Rules for Building-Related Products and
services, Part A: Calculation Rules for the Life Cycle
EN 15804+A2 Assesment and Requirements on the Project Report,
EN 15804+A2: Sustainability of construction works - March 2018
Environmental product declarations - Core rules for the
product category of construction products, 2019 PCR 2017, Part B
Institut Bauen und Umwelt e.V., Berlin (pub.): Product
IBU 2016 Category Rules for Construction Products from the
IBU (2016): General Programme Instructions for the range of Environmenal Product Declarations of Institut
Preparation of EPDs at the Institut Bauen und Umwelt Bauen und Umwelt (IBU), Part B: Requirements on the
e.V., Version 1.1 Institut Bauen und Umwelt e.V., EPD for insulating materials made of foam plastics.
Berlin, www.ibu-epd.de June 2017
6 Environmental Product Declaration Kingspan Insulation B.V. – Kooltherm® K15
REACH
Regulation (EC) No 1907/2006 of the European
Parliament and of the Council on the Registration,
Evaluation, Authorisation and Restriction of Chemicals
(REACH)
https://echa.europa.eu/candidate-list-table; accessed
19th of January 2021, 211 substances listed.
Renewable Energy Certificate
Towarowa Gielda Energii S.A.: Guarantees of origin
Document ID: RGP_ACTBV_2019-12-31_0720
7 Environmental Product Declaration Kingspan Insulation B.V. – Kooltherm® K15
Publisher
Institut Bauen und Umwelt e.V. Tel +49 (0)30 3087748- 0
Panoramastr. 1 Fax +49 (0)30 3087748- 29
10178 Berlin Mail info@ibu-epd.com
Germany Web www.ibu-epd.com
Programme holder
Institut Bauen und Umwelt e.V. Tel +49 (0)30 - 3087748- 0
Panoramastr 1 Fax +49 (0)30 – 3087748 - 29
10178 Berlin Mail info@ibu-epd.com
Germany Web www.ibu-epd.com
Author of the Life Cycle
Assessment Tel +31 (0) 543 543 210
Kingspan Insulation B.V. Fax +31 (0) 344 675 251
Lingewei 8 Mail info@kingspaninsulation.nl
4004LL Tiel Web www.kingspan.com
Netherlands
Owner of the Declaration
Kingspan Insulation B.V. Tel +31 (0) 543 543 210
Lingewei 8 Fax +31 (0) 344 675 251
4004LL Tiel Mail info@kingspaninsulation.nl
Netherlands Web www.kingspan.com
