ENVIRONMENTAL PRODUCT DECLARATION
as per ISO 14025 and EN 15804+A2
Owner of the Declaration Lanxess Deutschland GmbH, BU Inorganic Pigments
Publisher Institut Bauen und Umwelt e.V. (IBU)
Programme holder Institut Bauen und Umwelt e.V. (IBU)
Declaration number EPD-LAN-20230194-IBC2-EN
Issue date 10.08.2023
Valid to 09.08.2028
Iron Oxide Black Pigment (Fe3O4)
Lanxess Deutschland GmbH
www.ibu-epd.com | https://epd-online.com
1. General Information
Lanxess Deutschland GmbH Iron Oxide Black Pigment (Fe3O4)
Programme holder Owner of the declaration
IBU – Institut Bauen und Umwelt e.V. Lanxess Deutschland GmbH, BU Inorganic Pigments
Hegelplatz 1 Rheinuferstr. 7 - 9
10117 Berlin 47829 Krefeld
Germany Germany
Declaration number Declared product / declared unit
EPD-LAN-20230194-IBC2-EN 1,000 kg iron oxide black pigment
(weighted average)
This declaration is based on the product category rules: Scope:
Inorganic Pigments in Various Forms of Delivery, 01.08.2021 This EPD applies to iron oxide black pigments in the versions compacted,
(PCR checked and approved by the SVR) powder, granulate and micronized. It is an average EPD for which the
weighted average of the four versions was calculated on the basis of the
mass-specific production rate of the year 2021. Production of the pigments
Issue date in one single factory in Germany was assessed.
10.08.2023
The owner of the declaration shall be liable for the underlying information
and evidence; the IBU shall not be liable with respect to manufacturer
information, life cycle assessment data and evidences.
Valid to
09.08.2028 The EPD was created according to the specifications of EN 15804+A2. In
the following, the standard will be simplified as EN 15804.
Verification
The standard EN 15804 serves as the core PCR
Independent verification of the declaration and data according to ISO
14025:2011
internally X externally
Dipl.-Ing. Hans Peters
(Chairman of Institut Bauen und Umwelt e.V.)
Florian Pronold Matthias Klingler,
(Managing Director Institut Bauen und Umwelt e.V.) (Independent verifier)
1 Environmental Product Declaration - Lanxess Deutschland GmbH - Iron Oxide Black Pigment (Fe3O4)
2. Product
additives used must comply with EN 934-1, annexe A.1.
2.1 Product description/Product definition
Inorganic pigments are defined as substances that are The extremal values (worst-case assessment) across the three
insoluble in the application medium (ISO 18451-1) and assessed versions are used to prove conformity with the
manufactured by means of chemical synthesis. This EPD standard.
covers the product iron oxide black pigment in its typical
versions, namely powder, granulate, compacted and Performance figures for the product in line with the declaration
micronized. of performance in relation to its key characteristics as per DIN
EN 12878:2014 Pigments for the colouring of building materials
The average values of the inorganic pigments declared here based on cement and/or lime - Specifications and methods of
are based on the product volume in the indicated versions. test.
Regulation (EU) no. 305/2011 (CPR) applies to the placing of 2.4 Delivery status
the product on the market in the EU/EFTA (except Switzerland). Typical versions of the iron oxide black pigment are powder,
The product requires adeclaration of performance with due compacted, granulate and micronized. The packaging typically
consideration of DIN EN 12878:2014 Pigments for the coloring ranges from 25 kg polyethylene (PE)/paper sacks to big bags
of building materials based on cement and/or lime - with a net weight of one metric ton. The calculations in this EPD
Specifications and methods of test, and CE marking.The are based on an assessment of big-bag material. As the
respective national provisions apply to use. packaging material accounts for a very small proportion of the
calculated environmental impacts, only big bags made from
2.2 Application polypropylene (PP) and low-density polyethylene (LDPE) were
Inorganic iron oxide pigments are used for colouring building assessed as the packaging material.
materials made from cement, cement/lime mixtures, lime
mortar, and bituminous applications. Other applications include 2.5 Base materials/Ancillary materials
use in paints and coatings as well as plastics. On average, iron oxide black pigment is made up of the
following raw and auxiliary materials:
2.3 Technical Data
Name Value Unit
The product technical data that comes within the scope of the
Iron scrap 25,8 %
EPD is set out in the table below, with reference to the check
rules based on EN 12878. Nitrobenzene 21,6 %
Ferrous sulfate 14,7 %
Structural data - Influence on cement properties Direct reduced iron 12,8 %
Name Value Unit Sodium hydroxide 12,2 %
Setting time (start of setting process min. 1h) 177 min Iron (II) chloride 10,2 %
Setting time (end of setting time max. 12h) 269 min Sulphuric acid 0,3 %
Influence on cement setting (delta mixture with Hydrochloric acid 0,1 %
22 min
and without pigment max. + 60 min.) Phosphoric acid 0,1 %
Compressive strength (mortar 28 days (compare Cooling water 2,1 %
-0.6 N/mm2
mixture with and without pigment)) (category A)
1) The product/at least one partial product contains substances
Compressive strength (mortar 28 days (compare on the ECHA list of substances of very high concern (SVHC)
mixture with and without pigment)) (category B, 0.9 N/mm2 (date July 8, 2021) above 0.1 % by mass: No.
max. -8%)
Chloride content (total chloride; category A) 0.08 % 2)The product/at least one partial product contains further
Chloride content (total chloride; category B, max. carcinogenic, mutagenic, reprotoxic (CMR) substances in
0.06 %
0.1%) category 1A or 1B that are not on the candidate list, above 0.1
% by mass in at least one partial product: No.
Soluble chloride content (category A) 0.05 %
Soluble chloride content (total chloride; category
0.03 % 3) This construction product has had biocidal products added to
B, max. 0.1%)
it, or it has been treated with biocidal products (it is therefore a
Content of water-soluble substances (category 1.57 % treated article as per the Biocidal Products Regulation (EU) no.
A) 528/2012): No
Content of water-soluble substances (category
B, max. 0.5%) 1.62 % 2.6 Manufacture
The product is manufactured using the Laux process, which
*) Provided that the water-soluble content complies with EN
yields high-quality iron oxide pigments by reducing
934-1.
nitrobenzene with iron. Cast-iron filings, a waste product in the
steel-processing industry, are used as a raw material.
The amount of water-soluble substances as defined by EN 934-
The exothermic reaction is controlled in such a way that Fe O
1, paragraph 5.2.3, must not exceed: 3 4
is obtained.
• Category A: the level stated by themanufacturer
• Category B: 0.5 % by mass for individualpigments and
4 C H NO + 9 Fe + 4 H O → 4 C H NH + 3 Fe O
6 5 2 2 6 5 2 3 4
pigment mixtures. If additives such as dispersants,
binders, and/or grinding aids are used for powder or
The aniline is removed from the reaction mixture via steam
non-powder preparations, their water-soluble total
distillation. The residual iron is separated by means of a
content must be equal to or less than 5.5 % by mass
centrifugal separator. The remaining mixture is concentrated
(8.0 % for carbon black) in relation to the solid.The
2 Environmental Product Declaration - Lanxess Deutschland GmbH - Iron Oxide Black Pigment (Fe3O4)
further and washed in order to separate soluble components. The product is not a hazardous substance (as per the CLP
Regulation). There is no risk if the product is handled and
2.7 Environment and health during manufacturing
processed in compliance with the applicable regulations in the
LANXESS is continuously investing in modern manufacturing workplace.
processes at all locations. The Inorganic Pigments business
unit and its equipment are certified according to ISO 9001, 2.12 Reference service life
14001, and 50001. This EPD assesses modules A1–A3 (cradle to gate). The
service life corresponds to typical use in the respective
Iron oxide pigments are certified by SCS Global Services for application
their high content of recycled raw materials.
2.13 Extraordinary effects
2.8 Product processing/Installation Fire
As this EPD assesses modules A1–A3 (cradle to gate); a rough Fe O is non-flammable.
3 4
description of the application processes is attached.
Water
Customers typically use dosing units to dose iron oxide
No hazardous substances are released as a result of contact
pigments into specific colour mixtures and to process them into
with water.
cement-bound, lime-bound, or bituminous products.
Mechanical destruction
2.9 Packaging
Not applicable.
All versions of the pigments are packaged identically. The
finished product is usually packaged in PE/paper sacks with a 2.14 Re-use phase
net weight of 25 kg through to big bags made of PP and LDPE
This EPD assesses modules A1–A3 (cradle to gate). As iron
with a net weight of one metric ton.
oxide black pigments are bound in the application medium,
reuse is not pursued on account of the substantial amount of
According to the German Association for Plastics Packaging
thermal energy required and the technical options currently
and Films (IK), the big bags made of PP and LDPE on which
available. Recycling management provides individual
the calculations of the EPD are based can be reused in a
opportunities for the use of the bound pigment.
closed-loop system under specific conditions for the same
product (max. 2 years). The big bags can be recycled at the 2.15 Disposal
end of their life. For mechanical recycling, the used synthetic Disposal is carried out in conjunction with and in accordance
fabrics are treated mechanically with no change to the chemical with the respective application medium.
structure. The recycled materials can be used in various The waste code for iron oxide is 060316 (as per the German
applications and replace new granulate. Waste Catalog Ordinance).
2.10 Condition of use 2.16 Further information
This EPD assesses modules A1–A3 (cradle to gate). No Further information on iron oxide black pigments and further
material changes are expected within the recommended usage Lanxess IPG products and services is available at
limits. www.bayferrox.com
2.11 Environment and health during use
3. LCA: Calculation rules
A1: Supply of raw materials
3.1 Declared Unit A2: Transportation of raw materials to the manufacturer
The selected declared unit relates to an average product. The A3: Manufacture of the product (including required energy and
average was formed as a weighted mean from the annual water) and manufacture of the product packaging
production quantities of the compacted, powder, granulate and
micronized versions in the year 2021 (reference to mass). The use and disposal phase is not taken into accounting the
Declared unit and mass reference LCA calculations.
Name Value Unit 3.3 Estimates and assumptions
Declared unit 1000 kg Primary data across all versions were used for the
transportation of the iron filings (module A2) and for on-site
production processes at Lanxess Deutschland GmbH (module
3.2 System boundary A3). A distance of 1,000 km (within Europe) was assumed for
Type of EPD: Cradle to gate with options transportation of all further input materials (module A2).
Only modules A1 to A3 were calculated because the pigment Electricity consumption of 0.072 MJ per tkm was assumed for
fulfills all of the below criteria, as stated in PCR Part A: transportation via pipeline.
• the product is physically integrated with other products
Generic data was used for the production of raw materials
during installation so they cannot be physically
(module A1) as these are not produced by Lanxess
separated from them at the end of life,
Deutschland GmbH itself and no detailed information was
• the product is no longer identifiable at the end of life as
available.
a result of a physical or chemical transformation
process,
Credits for the avoidance of generation of electricity and steam
• the product does not contain biogenic carbon.
in another product system through the incineration processes
for production waste were also taken into account (module D).
The following modules were taken into account in the LCA
100 % incineration including energy recovery (electricity and
calculation
steam) was assumed here.
3 Environmental Product Declaration - Lanxess Deutschland GmbH - Iron Oxide Black Pigment (Fe3O4)
weighting for the average assessment.
3.4 Cut-off criteria
All primary data of the production processes were taken into 3.8 Geographic Representativeness
account. No cut-off rules were applied. Land or region, in which the declared product system is
manufactured, used or handled at the end of the product´s
3.5 Background data lifespan: Germany
The software system GaBi 10 developed by Sphera was used
for modelling the product's LCA. The data sets contained
therein are either from the GaBi Professional database (v 3.9 Allocation
2023.1) or from the Ecoinvent database (v 3.8). For the iron fillings (iron scrap) used, only the expenses for
treatment are taken into account in module A1 as they relate to
3.6 Data quality pre-consumer material as per ISO 14021.
The GaBi software system for life-cycle analyses and the GaBi
Professional database (v 2023.1), as well as the Ecoinvent Aniline is a co-product in the manufacture of the ironoxide black
database (v 3.8) were used for the life-cycle modeling of the pigment. In line with the requirements of EN15804 (section
assessed products. The produced quantities for 2021 were 6.4.3.2), an allocation based on physical properties (mass) was
gathered by Lanxess. carried out in modules A1 and A3. 71 % of the material flows
were assigned to the product.
Corresponding data sets were available for the input materials
used, and some of them have been adapted with regard to All credits from recovered energy from processes relating to the
concentration. The age of the background data used (2018– incineration of production waste were allocated to module A3
2021) is less than 15 years and can be regarded as with the closed-loop method.
representative for the assessment period.
3.10 Comparability
The LCA figures for the average EPD (weighted mean for the Basically, a comparison or an evaluation of EPD data is only
year 2021) can be regarded as robust as they are a weighted possible if all the data sets to be compared were created
average of high-quality, measured activity data. All data used according to EN 15804 and the building context, respectively
can be regarded as representative. the product-specific characteristics of performance, are taken
into account. Background data was taken from the GaBi
3.7 Period under review Professional database (v 2023.1). To fill occasional gaps,
The assessment period is 2021. All in-house data was gathered datasets from the Ecoinvent database (v 3.8) were used.
in this period and then correspondingly subjected to average
4. LCA: Scenarios and additional technical information
Characteristic product properties of biogenic carbon As disposal of the packaging material on the buildingsite
The content of biogenic carbon in the product is 0 % and is (module A5) is not declared, the assessed quantities of
therefore not reported separately. The product packaging packaging materials are stated below:
consists of plastic (PP) without biogenic content.
• Big bag (PP): 2.05 kg/1,000 kg product
• Big bag (LDPE): 0.72 kg/1,000 kg product
Technical Information
Module D comprises the credits for the incineration processes
(i.e. credits for electricity and steam as aresult of incineration of
The following technical information forms the basis for the
production waste). The credits are based on German average
declared modules or can be used to develop specific scenarios
data for electrical and thermal energy.
in the context of a building assessment if modules are not
declared (MND).
4 Environmental Product Declaration - Lanxess Deutschland GmbH - Iron Oxide Black Pigment (Fe3O4)
5. LCA: Results
The following tables show the environment-relevant results as per EN 15804 for 1,000 kg iron oxide black pigment (weighted average
for the compacted, powder, granulate and micronized versions).
DESCRIPTION OF THE SYSTEM BOUNDARY (X = INCLUDED IN LCA; ND = MODULE OR INDICATOR NOT DECLARED; MNR =
MODULE NOT RELEVANT)
Benefits and
Construction loads beyond
Product stage Use stage End of life stage
process stage the system
boundaries
la ire ta m w a Ry lp p u s tro p s n a rT g n iru tc a fu n a M e h t m o rf tro p s n a rTe tis e h t o t e ta g y lb m e s s A e s U e c n a n e tn ia M ria p e R tn e m e c a lp e R tn e m h s ib ru fe R y g re n e la n o ita re p Oe s u re ta w la n o ita re p Oe s u n o itc u rts n o c -e Dn o itilo m e d tro p s n a rT g n is s e c o rp e ts a W la s o p s iD -e s u e R-y re v o c e R-g n ilc y c e Rla itn e to p
A1 A2 A3 A4 A5 B1 B2 B3 B4 B5 B6 B7 C1 C2 C3 C4 D
X X X MND MND MND MND MNR MNR MNR MND MND MND MND MND MND MND
RESULTS OF THE LCA - ENVIRONMENTAL IMPACT according to EN 15804+A2: 1000 kg Iron oxide black pigment
Parameter Unit A1-A3 A1 A2 A3
Global Warming Potential total (GWP-total) kg CO 2 eq 1.77E+03 9.97E+02 1.37E+02 6.4E+02
Global Warming Potential fossil fuels (GWP-fossil) kg CO 2 eq 1.69E+03 9.9E+02 1.37E+02 5.61E+02
Global Warming Potential biogenic (GWP-biogenic) kg CO 2 eq 8.51E+01 6.32E+00 -4.83E-01 7.93E+01
Global Warming Potential luluc (GWP-luluc) kg CO 2 eq 9.61E-01 4.15E-01 5.16E-01 3.02E-02
Depletion potential of the stratospheric ozone layer (ODP) kg CFC11 eq 4.29E-06 4.29E-06 1.05E-10 6.54E-10
Acidification potential of land and water (AP) mol H+ eq 3.04E+00 2.18E+00 3.58E-01 4.97E-01
Eutrophication potential aquatic freshwater (EP-freshwater) kg P eq 3.26E-02 3.22E-02 2.82E-04 1.13E-04
Eutrophication potential aquatic marine (EP-marine) kg N eq 9.85E-01 6.32E-01 1.62E-01 1.9E-01
Eutrophication potential terrestrial (EP-terrestrial) mol N eq 1.07E+01 6.73E+00 1.82E+00 2.11E+00
kg NMVOC
Formation potential of tropospheric ozone photochemical oxidants (POCP) 2.64E+00 1.78E+00 3.29E-01 5.26E-01
eq
Abiotic depletion potential for non fossil resources (ADPE) kg Sb eq 1.14E-03 1.09E-03 1.5E-05 3.07E-05
Abiotic depletion potential for fossil resources (ADPF) MJ 3.07E+04 2.07E+04 1.82E+03 8.16E+03
m3 world eq
Water use (WDP) 4.28E+01 2.13E+01 6.54E-01 2.08E+01
deprived
RESULTS OF THE LCA - INDICATORS TO DESCRIBE RESOURCE USE according to EN 15804+A2: 1000 kg Iron oxide black
pigment
Parameter Unit A1-A3 A1 A2 A3
Renewable primary energy as energy carrier (PERE) MJ 1.59E+03 1.25E+03 1.18E+02 2.28E+02
Renewable primary energy resources as material utilization (PERM) MJ 0 0 0 0
Total use of renewable primary energy resources (PERT) MJ 2.34E+03 1.25E+03 1.18E+02 9.71E+02
Non renewable primary energy as energy carrier (PENRE) MJ 3.06E+04 2.16E+04 1.24E+03 7.78E+03
Non renewable primary energy as material utilization (PENRM) MJ 1.21E+02 0 0 1.21E+02
Total use of non renewable primary energy resources (PENRT) MJ 3.07E+04 2.16E+04 1.24E+03 7.9E+03
Use of secondary material (SM) kg 0 6.12E+02 0 0
Use of renewable secondary fuels (RSF) MJ 0 0 0 0
Use of non renewable secondary fuels (NRSF) MJ 0 0 0 0
Use of net fresh water (FW) m3 3.73E+00 2.75E+00 7.61E-02 9.06E-01
RESULTS OF THE LCA – WASTE CATEGORIES AND OUTPUT FLOWS according to EN 15804+A2:
1000 kg Iron oxide black pigment
Parameter Unit A1-A3 A1 A2 A3
Hazardous waste disposed (HWD) kg 5.01E+01 3.2E+01 5.89E+00 1.22E+01
Non hazardous waste disposed (NHWD) kg 2.25E+01 9.69E+00 2.3E-01 1.26E+01
Radioactive waste disposed (RWD) kg 5.05E+01 3.22E+01 5.9E+00 1.25E+01
Components for re-use (CRU) kg 0 0 0 0
Materials for recycling (MFR) kg 0 0 0 0
Materials for energy recovery (MER) kg 0 0 0 0
Exported electrical energy (EEE) MJ 0 0 0 0
Exported thermal energy (EET) MJ 0 0 0 0
RESULTS OF THE LCA – additional impact categories according to EN 15804+A2-optional:
1000 kg Iron oxide black pigment
Parameter Unit A1-A3 A1 A2 A3
Disease
Incidence of disease due to PM emissions (PM) ND ND ND ND
incidence
Human exposure efficiency relative to U235 (IR) kBq U235 eq ND ND ND ND
Comparative toxic unit for ecosystems (ETP-fw) CTUe ND ND ND ND
5 Environmental Product Declaration - Lanxess Deutschland GmbH - Iron Oxide Black Pigment (Fe3O4)
Comparative toxic unit for humans (carcinogenic) (HTP-c) CTUh ND ND ND ND
Comparative toxic unit for humans (noncarcinogenic) (HTP-nc) CTUh ND ND ND ND
Soil quality index (SQP) SQP ND ND ND ND
Disclaimer 1 – for the indicator “Potential Human exposure efficiency relative to U235”. This impact category deals mainly with the
eventual impact of low-dose ionizing radiation on human health of the nuclear fuel cycle. It does not consider effects due to possible
nuclear accidents, occupational exposure or radioactive waste disposal in underground facilities. Potential ionizing radiation from the
soil, radon and from some construction materials is also not measured by this indicator.
Disclaimer 2 – for the indicators “abiotic depletion potential for non-fossil resources”, “abiotic depletion potential for fossil resources”,
“water (user) deprivation potential, deprivation-weighted water consumption”, “potential comparative toxic unit for ecosystems”,
“potential comparative toxic unit for humans – cancerogenic”, “Potential comparative toxic unit for humans - not cancerogenic”,
“potential soil quality index”. The results of this environmental impact indicator shall be used with care as the uncertainties on these
results are high as there is limited experience with the indicator.
6. LCA: Interpretation
The product is evaluated below for the weighted average of the
four versions, namely compacted, powder, granulate and
micronized.
The largest share of the gross energy demand is attributed in
each case to the production of the raw materials (A1) (approx.
22,800 MJ, 71 %). The transport of the raw materials requires
approx. 4 % of the energy expenditures (A2), while the
production process accounts for a share of 25 %.
In the production of the raw materials for the black pigment,
nitrobenzene, the iron sponges (Direct Reduced Iron) or the
sodium hydroxide are also decisive for the environmental
impact, depending on the delivery form. For more details
between the four delivery forms see the results in the annex.
In Module A3 (manufacturing process), the environmental
The environmental impact categories are significantly impacts are essentially dominated by the use of electricity and
influenced (at least 50 %) by the provision of raw materials natural gas. The only exceptions are the categories Climate
(module A1). The only exceptions are the categories Climate Change, Biogenic and Water Removal Potential (WDP), which
Change, Biogenic and Land Use, where the greatest influence mainly reflect the incineration of industrial waste.
lies in the manufacturing processes (Module A3) or in the
transport of the input materials (Module A2). When interpreting the results, it should be noted that various
assumptions and estimates were made. This mainly concerns
With the exception of the Climate Change, Land Use category, the transports to the plant. It can be assumed that the influence
the transportation processes do not have a significant impact on the overall result is not significant even with variations in the
on the environmental impact of the products. The share of the assumptions / estimates made, since transports do not have a
manufacturing processes (A3) in the individual categories is major influence.
between 0 % and 49 % in all categories. In the impact category
Climate Change, biogenic, the influence is at 93 %.
7. Requisite evidence
No proof has to be provided for this EPD as no hazardous
substances as per the CLP Regulation are used.
6 Environmental Product Declaration - Lanxess Deutschland GmbH - Iron Oxide Black Pigment (Fe3O4)
8. References
Standards BPR Regulation
Regulation (EU) No 528/2012 of the European Parliment and
EN 934-1 the Council of 22 May 2012 concerning the making available on
DIN EN 934-1:2008-04, Admixtures for concrete, mortar, and the market and use of the biocidal products (Text with EES
grout - Part 1: Common requirements. relevance)
EN 12878 SCS Global Services
DIN EN 12878:2014, Pigments for the coloring of building Scientific Certification Systems.
materials based on cement and/or lime -Specifications and https://www.scsglobalservices.com/
methods of test.
German Waste Catalog Ordinance (AVV)
EN 15804 Ordinance on the European List of Waste, Waste Catalog
DIN EN 15804:2012-04+A1 2013, Sustainability of construction Ordinance dated December 10, 2001 (German Federal Gazette
works – Environmental product declarations – Core rules for the I p. 3379), last amended by Article 1of the Ordinance dated
product category of construction products. June 30, 2020 (German Federal Gazette I p. 1533).
ISO 9001 CLP Regulation
DIN EN ISO 9001:2015, Quality management systems– Regulation (EG) no. 1272/2008 of the European Parliament
Requirements. and of the Council of December 16, 2008,on classification,
labeling, and packaging of substances and mixtures, amending
ISO 14001 and repealing Directives 67/548/EEC and 1999/45/EC,
DIN EN ISO 14001:2015, Environmental management andamending Regulation (EC) no. 1907/2006 (Official Journal L
systems - Requirements with guidance for use. 353 dated December 31, 2008, p. 1–1355), last amended by
Delegated Regulation (EU)2021/1962 of the Commission dated
ISO 14021 August 12, 2021 (Official Journal L 400/16).
DIN EN ISO 14021:2016, Environmental labels and
declarations – Self-declared environmental claims (Type II Ecoinvent database
environmental labeling). Ecoinvent database version 3.8, 2021
ISO 14025 GaBi Professional database
DIN EN ISO 14025:2011-10, Environmental labels and GaBi Professional database version 10.2, 2022
declarations – Type III environmental declarations –Principles
and procedures. IBU 2021
Institut Bauen und Umwelt e.V.: General guide for the EPD
ISO 18451-1 program of the Institut Bauen und Umwelt e.V.(IBU). Version
DIN EN ISO 18451-1:2019, Pigments, dyestuffs, and 2.0, Berlin: Institut Bauen und Umwelt e.V., 2021.www.ibu-
extenders - Terminology - Part 1: General terms. epd.com
ISO 50001 PCR part A
DIN EN ISO 50001:2018, Energy management systems - Product category rules for building-related productsand
Requirements with guidance for use. services. Part A: Calculation rules for the LCA and
requirements for the background report, v. 2.0. Berlin:Institut
Further literature Bauen und Umwelt e.V. (publisher), 2021.
CPR Regulation PCR: Inorganic pigments in different versions
Regulation (EU) No 305/2011 of the European Parliament and Product category rules for building-related productsand
of the Council of March 2011, laying down harmonised services. Part B: Requirements for the EPD for inorganic
conditions for the marketing of construction products and pigments in different versions, v.1.0. Berlin: Institut Bauen und
repealing Council Directive 89/106/EEC Umwelt e.V. (publisher), 2021.
ECHA
European Chemicals Agency: Candidate List of substances of
very high concern, 2022
7 Environmental Product Declaration - Lanxess Deutschland GmbH - Iron Oxide Black Pigment (Fe3O4)
Publisher
Institut Bauen und Umwelt e.V. +49 (0)30 3087748- 0
Hegelplatz 1 info@ibu-epd.com
10117 Berlin www.ibu-epd.com
Germany
Programme holder
Institut Bauen und Umwelt e.V. +49 (0)30 3087748- 0
Hegelplatz 1 info@ibu-epd.com
10117 Berlin www.ibu-epd.com
Germany
Author of the Life Cycle Assessment
TÜV Rheinland Energy GmbH +49 (0)221 806 0
Am Grauen Stein 33 carbon@de.tuv.com
51105 Köln www.tuv.com
Germany
Owner of the Declaration
Lanxess Deutschland GmbH, BU Inorganic Pigments +49 221 8885 5179
Rheinuferstr. 7 - 9 uwe.hempelmann@lanxess.com
47829 Krefeld bayferrox.com
Germany
8 Environmental Product Declaration - Lanxess Deutschland GmbH - Iron Oxide Black Pigment (Fe3O4)
