ENVIRONMENTAL PRODUCT DECLARATION
as per ISO 14025 and EN 15804+A2
Owner of the Declaration IVPU - Industrieverband Polyurethan-Hartschaum e.V.
Publisher Institut Bauen und Umwelt e.V. (IBU)
Programme holder Institut Bauen und Umwelt e.V. (IBU)
Declaration number EPD-IVP-20240422-IBE1-EN
Issue date 29.11.2024
Valid to 28.11.2029
PU thermal insulation boards with 50 µm aluminium facing
IVPU e.V.
www.ibu-epd.com | https://epd-online.com
1. General Information
IVPU e.V. PU thermal insulation boards with 50 µm
aluminium facing
Programme holder Owner of the declaration
IBU – Institut Bauen und Umwelt e.V. IVPU ­ Industrieverband Polyurethan­Hartschaum e.V.
Hegelplatz 1 Heilbronner Str. 154
10117 Berlin 70191 Stuttgart
Germany Germany
Declaration number Declared product / declared unit
EPD­IVP­20240422­IBE1­EN 1 m² of installed PU thermal insulation board with 50 µm aluminium facing
(on both sides), a thickness of 12 cm, and a nominal thermal conductivity
of 0,022 W/(m.K) and delcared value of thermal resistance of R = 5,45
d
(m²•K)/W
This declaration is based on the product category rules: Scope:
Insulating materials made of foam plastics, 01.08.2021 This EPD applies to all declared products of the IVPU's member
(PCR checked and approved by the SVR) companies Karl Bachl GmbH & Co KG, Paul Bauder GmbH & Co KG, IKO
Insulation BV, Kingspan Insulation GmbH & Co KG, Linzmeier
Bauelemente GmbH, puren gmbh, Recticel NV/SA, Soprema GmbH,
Issue date Steinbacher Dämmstoff­GmbH, Unilin Insulation bv. The IVPU represents
more than 90% of the companies within the German polyurethane
29.11.2024
insulation products market. This EPD is based on weighted averages,
which have been determined on the basis of the single values originating
from the aforementioned manufacturing companies' factories (see section
Valid to
3.1).
28.11.2029 The owner of the declaration shall be liable for the underlying information
and evidence; the IBU shall not be liable with respect to manufacturer
information, life cycle assessment data and evidences.
The EPD was created according to the specifications of EN 15804+A2. In
the following, the standard will be simplified as EN 15804.
Verification
The standard EN 15804 serves as the core PCR
Independent verification of the declaration and data according to ISO
14025:2011
Dipl.­Ing. Hans Peters internally X externally
(Chairman of Institut Bauen und Umwelt e.V.)
Florian Pronold Prof. Dr. Birgit Grahl,
(Managing Director Institut Bauen und Umwelt e.V.) (Independent verifier)
1 Environmental Product Declaration ­ IVPU e.V. ­ PU thermal insulation boards with 50 µm aluminium facing
2. Product
Name Value Unit
2.1 Product description/Product definition
Gross density 31 ­ 32 kg/m3
Factory made rigid polyurethane foam (PU) products are used
for the thermal insulation of buildings. PU includes both PIR Compressive strength acc. to DIN 100 – 150 kPa
and PUR products. The products are manufactured in the form EN 826
of boards without or with flexible facings. Tensile strength to DIN EN 1607 ≥ 40 kPa
This Product Declaration covers PU insulation boards with 50 Modulus of elasticity acc. to DIN EN
≥ 4 N/mm2
µm aluminium facings on both sides. For the placing on the 826
market of the product in the European Union/European Free
Calculation value for thermal
Trade Association (EU/EFTA) (with the exception of 0.023 W/(mK)
conductivity
Switzerland) Regulation (EU) No. 305/2011 (CPR) applies. The
Water vapour diffusion resistance
product needs a declaration of performance taking into ∞ ­
factor acc. to EN 12088
consideration EN 13165:2016-09 Thermal insulation products
Dimensional stability under defined
for buildings ­ Factory made rigid polyurethane foam (PU) DS(70/90)3 and
temperature and humidity Class
products ­ Specification and the CE­marking. DS(­20,­)1
conditions DS(TH)i
For the application and use the respective national provisions Limiting dimensions of thickness Ti T2 Class
apply. In Germany, the design values for application in building Thermal conductivity acc. to DIN
0.022 W/(mK)
construction are specified in DIN 4108-10. Hygrothermal design EN 13165
values are regulated in DIN 4108-4. Calculation value for thermal
0.023 W/(mK)
conductivity (Deutschland)
2.2 Application
Creep behaviour or permanent
The scope of application of PU rigid foam insulation materials
compressive strength acc. to DIN ≥ 0.02 N/mm2
includes thermal insulation in building construction (e.g. pitched
EN 1606
roofs, flat roofs, floors, ceilings and exterior walls (inside and
outside). Declared value of thermal
5.45 (m²•K)/W
resistance RD
2.3 Technical Data Thickness at RD = 1 (m²•K)/W 22 mm
For determining technical data, testing methods as stated in
Performance data of the production in accordance with the
DIN EN 13165 are used. The gross density of PU insulation
declaration of performance with respect to its essential
boards with 50 µm aluminium facings for building construction
characteristics according to DIN 4108-10: 2021-11 (Table 6).
is approx. 31 ­ 32 kg/m³.
The nominal thermal conductivity is 0.022 W/(m.K), the thermal
2.4 Delivery status
conductivity design value which is used for calculating the
Polyurethane insulation boards with 50 µm aluminium facings
thermal performance of insulation layers in buildings is 0.023
are manufactured with plane­parallel surfaces or as tapered
W/(m.K). In addition, the nominal value of the thermal
insulation boards in a thickness range of 20 to 300 mm. This
resistance of R = 5.45 (m².K)/W and the thickness of 22 mm of
D Product Declaration refers to a board thickness of 120 mm. The
the insulation board at R = 1 (m².K)/W can be specified. format of the boards depends on the planned application. The
D
The Nominal compressive stress at 10% deformation or width can be up to 1250 mm and the length up to 12 m. This
compressive strength is 100 kPa (dh) or 150 kPa (ds) acc. to product declaration refers to a surface area of 1 m2.
DIN 4108-10. Higher compressive strength is possible. Nominal
2.5 Base materials/Ancillary materials
tensile strength perpendicular to the insulation board plane is
40 kPa. Higher tensile strength is possible. PU insulation The 12 cm PU board with 50 µm aluminium facings consists of
boards with 50 µm aluminium facings are impermeable to water 3.88 kg/m² PU rigid foam and 0.28 kg/m² 50 µm aluminium
vapour and do not absorb moisture. Polyurethane rigid foam is facings. Polyurethane rigid foam is formed by the chemical
a distinctive thermosetting material and therefore cannot be reaction of MDI (approx. 58 – 65 %) and polyol (approx. 26 –
melted. 31 %), adding low boiling point blowing agents (approx. 3 – 6
%). Insulation boards with flexible facings are foamed
Constructional data
exclusively with the hydrocarbon pentane. Due to the closed­
cell structure, the blowing agent remains within the foam cells.
Water (approx. 0.2 – 1.5 %), foam stabilisers and catalysts
(approx. 2 – 6 %), as well as flame retardants (Phosphoric acid
ester; approx. 2 – 5 %) are added as ancillary materials.
The raw materials used for the production of polyurethane rigid
foam are mainly obtained from crude oil, undergoing several
production stages. Alternatively, polyols and MDI can be
produced, in part, from renewable, plant­based raw materials or
recycled materials. This is not part of this EPD.
Polyurethane rigid foam does not contain volatile isocyanates.
Under the current Regulation on the Registration, Evaluation,
Authorisation and Restriction of Chemicals (REACH)
polyurethane rigid foam is declared as follows:
• Polyurethane rigid foam contains substances listed in
the Candidate List for authorization on 23 January 2024
2 Environmental Product Declaration ­ IVPU e.V. ­ PU thermal insulation boards with 50 µm aluminium facing
exceeding 0.1 percentage by mass: no. construction and does not rot.
• Polyurethane rigid foam contains other carcinogenic,
mutagenic, reprotoxic (CMR) substances in categories 2.11 Environment and health during use
1A or 1B which are not on the candidate list, exceeding The requirements of the Committee for Health­related
0.1 percentage by mass: no Evaluation of Building Products (AgBB) are met. Measurements
• Biocide products were added to this construction of emissions using testing chambers in accordance with the
product or it has been treated with biocide products (this relevant testing norms (EN 16516) showed that volatile organic
then concerns a treated product as defined by the (EU) substances (VVOC, VOC) are only emitted in small quantities.
Ordinance on Biocide Products No. 528/2012): no
50 µm aluminium facings consist of lacquered aluminium foil. Regarding the current REACH candidate list, the foam
formulations contain no SVHC substances (see section 2.5).
2.6 Manufacture
Polyurethane rigid foam insulation boards with flexible 50 µm Polyurethane insulaton products are odourless.
aluminium facings are produced in a continuous process on a
double belt line. In this process, the polyurethane reaction 2.12 Reference service life
mixture pours from a mixing head onto the bottom aluminium When used properly, the service life time of polyurethane rigid
facing where it foams up and glues – still within the line's foam corresponds to the service life time of the insulated
pressure area – with the top aluminium facing. After passing the construction component or building. The performance of the
double belt line, the foam boards are cut to the desired insulation boards stays the same throughout the entire service
dimensions. life time.
Description of the influences on the ageing of the product when
Quality assurance applied in accordance with the rules of technology.
The declared products are subject to quality controls. Quality
assurance is based on surveillance and certification by
2.13 Extraordinary effects
independent Notified Bodies.
Fire
2.7 Environment and health during manufacturing According to national approvals, polyurethane insulaton
No health protection measures extending beyond the legally­ materials are classified either as class E or class C acc. to EN
mandated work protection measures for industrial businesses 13501-1. Pitched roof constructions with polyurethane
are required during the entire manufacturing process. No insulation over rafters that comply with the classification report
special environmental protection measures apart from the legal of IBS 316052507-A are classified as REI 30 (fire­retardant).
provisions are required. Roof structures with top­side polyurethane insulation acc. to
DIN 18234-2 meet the fire­protection requirements stated in the
2.8 Product processing/Installation Industrial Building Guideline even for fire containment or fire
Polyurethane insulation boards can be cut, sawed, milled, and fighting sections with a roof surface of more than 2500 m².
abraded with conventional construction tools and portable
machines. In general, the boards are fixed mechanically In case of fire, PU rigid foam does not tend to smoulder. When
(pitched and flat roofs, cavity core insulation). Alternatively, PU exposed to heat, PU rigid foam carbonizes without dripping off
insulation boards can be laid loosely, e.g. on floors. Observing burning droplets. When burning, sooty products, water vapour,
the manufacturer's recommendations, it is also possible to glue carbon monoxide, carbon dioxide, nitrogen oxides, as well as
the boards together by using either hot­setting or cold­setting hydrogen cyanide are formed as it is the case e. g. for sheep
adhesives. Joints between cut insulation boards on roof ridges, wool.
hips or valleys are to be sealed with polyurethane in­situ foam The toxicity of the combustion gases mainly depends on the
without thermal bridges. amount of burned material in relation to the size of the room in
which the gases are distributed. It also depends on the
While sawing, abrading, and milling insulation boards, dust is ventilation conditions in the affected area.
generated. If there is no sufficient ventilation, workers who carry
out these processes have to protect themselves by wearing an
Fire protection
appropriate dust filter mask (see leaflet of the
Name Value
'Berufsgenossenschaft der Chemischen Industrie'
on respiratory protection). Dust concentration in the air (general Building material class acc to EN 13501 E ­ C
limit of dust concentration as per TRGS 900, Technische Burning droplets d0, none
Regeln für Gefahrstoffe) must not exceed the following values: Smoke gas development s1 ­ s3
• 10 mg/m³ (measured as inhalable fraction)
• 1.25 mg/m³ (measured as alveolar fraction) Water
These limits are time­weighted averages assuming an 8­hour Due to the predominant closed­cell structure, insulation
exposure per day, 5 days a week, during working lifetime. materials made of polyurethane rigid foam absorb water only in
Cutting leftovers can be treated in a municipal waste small quantities. They are not hygroscopic, i.e. they do not
incernation plant with energy recovery or they can be subject to absorb water vapour from the air. When unexpectedly exposed
a separate collection and a mechanical recycling process. to water (e.g. flood), only very small amounts of soluble
substances are emitted.
2.9 Packaging
Mainly, plastic foils and EPS or PU wedges are used as
Mechanical destruction
packaging material. The plastic foils can be recycled whereas
The disintegration of the poduct by mecanical processes does
the PU wedges can be reused in the form of PU press plates.
not have relevant effects on the environment.
2.10 Condition of use
2.14 Re-use phase
Under normal conditions of use, the material does not undergo
Dismantling polyurethane insulation products as well as sorting
any changes in terms of substance during its service life time.
and waste identifying can be done without difficulties, since
Polyurethane is resistant to most chemicals used in
they are usually mounted mechanically or laid loosely.
3 Environmental Product Declaration ­ IVPU e.V. ­ PU thermal insulation boards with 50 µm aluminium facing
material that are used, among others, to insulate window
Clean and undamaged polyurethane insulation boards can be frames or thermal bridges.
reused as well as recycled mechanically or chemically
(glycolysis). Glycolysis means that polyurethane rigid foam 2.15 Disposal
waste is transformed into a fluid substance called glycolysis According to the Waste Catalogue Ordinance, polyurethane
polyol, which can be used again as raw material in the insulating material shall not be disposed of without prior
production of polyurethane. treatment. The waste code for construction waste is 170604.
During thermal treatment, the energy content of the insulation
When reutilised from mechanical material recycling, material can be recovered.
polyurethane rigid foam waste is used to produce press boards.
2.16 Further information
In this process, cutting and mounting leftovers, as well as
construction waste, are mechanically shredded and Please visit www.ivpu.de and www.daemmt­besser.de for
subsequently pressed into board­shaped products while adding further information on PU insulation products.
binding agents. PU pressed adhesive boards are a high­quality
3. LCA: Calculation rules
Using a worst­case approach, only the incineration and the
3.1 Declared Unit consequent energy benefits beyond the system boundary have
The declared unit is 1 m² of installed PU thermal insulation been considered in this EPD.
board with 50 µm aluminium facing (on both sides) and has the
following specifications: 3.4 Cut-off criteria
In this study, all available data from the production are taken
Declared unit
into account, i.e. all used raw materials, used thermal energy,
Name Value Unit
as well as electrical power consumption. Therefore, even
Declared unit 1 m2 materials and power consumption levels that have a share of
Gross density of PU foam 32.29 kg/m3 less than 1 % are considered.
Grammage 4.15 kg/m2
It can be assumed that all neglected processes put together
Layer thickness 0.12 m
account for no more than 5 % of total power and mass
Design value of thermal conductivity 0.023 W/(m•K) consumption. The manufacturers have provided data on
Thermal resistance (R­value) 5.45 m²·W/K transport expenditures for all relevant material flows. Machinery
and installations required for production are neglected.
Other declared units are allowed if the conversion is shown
transparently. 3.5 Background data
Background data originates from the Sphera LCA FE (GaBi ts)
This EPD is based on weighted averages, which have been
software database CUP 2023.2 from Sphera. The power mix
determined on the basis of the single values originating from
with different countries has been used. The last revision of the
the factories of the IVPU members. Average energy
used data was less than 6 years ago.
consumption for producing PU boards has been weighted
according to the quantities of produced PU rigid foam in m3. 3.6 Data quality
Raw material consumption has been weighted according to The data used are primary data originating from the industry
used quantities in kg. Rigid foam waste is weighted according and were gathered by the IVPU in 2018. 9 IVPU members
to the quantities of produced PU rigid foam in m3 whereas participated in this data gathering. The IVPU represents more
facing waste is weighted according to used quantities of facings than 90 % of the companies within the German polyurethane
in m2. insulation products market. This EPD is based on weighted
averages, which have been determined on the basis of the
3.2 System boundary single values originating from the factories of the afore­
The type of EPD according to EN15804 is cradle to gate with mentioned manufacturing companies.
options, modules C1–C4, and module D. The data's quality as well as its temporal, technological and
Life cycle assessment considers the following steps of the life geographical representativeness significance can be classified
cycle: as good.
• Production and supply of raw materials (A1)
3.7 Period under review
• Transporting raw materials (A2)
The data basis is based on production data from 2018.
• Production expenses including packaging (A3)
The used quantities of raw materials, energy, as well as
• Transport to construction site (A4)
ancillary materials and fuels are averages compiled over a time
• Installation in buildings (thermal treatment of packaging
span of 12 months.
waste) (A5)
• Transport to End­of­Life (C2)
3.8 Geographic Representativeness
• Waste treatment: energy for shredders (C3)
Land or region, in which the declared product system is
• Thermal treatment (PU foam) (C3)
manufactured, used or handled at the end of the product´s
• Recycling or use potentials beyond the system's
lifespan: Germany
boundary (D).
3.3 Estimates and assumptions
3.9 Allocation
For all inputs, specific Sphera LCA FE (GaBi ts) datasets were
When thermally treated in waste incineration plants, recycling
available.
as well as use potentials beyond the system boundary for
Currently, waste from PU foam production generated in
power and thermal energy in module D are taken into account
construction sites are handled using mainly material recycling
in an input­specific manner considering elemental composition
(see 2.15).
as well as thermal values. Due to manufacturing locations and
4 Environmental Product Declaration ­ IVPU e.V. ­ PU thermal insulation boards with 50 µm aluminium facing
distribution throughout all of Europe, the substitution processes according to EN 15804 and the building context, respectively
refer to reference area EU­27. the product­specific characteristics of performance, are taken
into account. The used background database is Sphera LCA
3.10 Comparability FE (GaBi ts), CUP 2023.2.
Basically, a comparison or an evaluation of EPD data is only
possible if all the data sets to be compared were created
4. LCA: Scenarios and additional technical information
Installation in buildings (A5)
Characteristic product properties of biogenic carbon
The biogenic carbon content declared is provided below. No Name Value Unit
biogenic carbon content exists in the product, only packaging Packaging waste 0.68 kg
materials.
Information on describing the biogenic carbon content at
End of life cycle (C1-C4)
factory gate
Name Value Unit
Name Value Unit
Waste processing (C3) energy for shredders 0.83 MJ
kg
Biogenic carbon content in product ­ Reuse ­ kg
C
Recycling (aluminium) 0.28 kg
Biogenic carbon content in accompanying kg
packaging 0.0744 C Energy recovery 3.87 kg
Landfilling ­ kg
Note: 1 kg of biogenic carbon is equivalent to 44/12 kg of CO2.
Module C1 considers a manual demolition (without any
burden). Upon removal from the building, products are
The following technical scenario information is used to calculate assumed to be transported 100 km (module C2) to a recycling
the declared modules.The values refer to the declared unit of 1 facility. The foam waste in the EoL phase is sent to a waste
m² of installed PU thermal insulation board with 50 µm incineration plant.
aluminium facing.
The waste is shredded and incinerated. These processes are
Transport to construction site (A4)
grouped to module C3. Resulting potential benefits for
Name Value Unit
electricity and thermal energy due to the incineration are
Litres of fuel 0.027 l/100km grouped to module D.
Transport distance 500 km
Gross density of products transported 32.29 kg/m3 Aluminum facings are recycled. The recycling including the
recycling effort and the potential benefits are addressed in
Capacity utilisation (including empty runs) 85 %
module D.
5 Environmental Product Declaration ­ IVPU e.V. ­ PU thermal insulation boards with 50 µm aluminium facing
5. LCA: Results
DESCRIPTION OF THE SYSTEM BOUNDARY (X = INCLUDED IN LCA; MND = MODULE OR INDICATOR NOT DECLARED; MNR
= MODULE NOT RELEVANT)
Benefits and
Construction loads beyond
Product stage Use stage End of life stage
process stage the system
boundaries
la ire ta m w a Ry lp p u s tro p s n a rT g n iru tc a fu n a M e h t m o rf tro p s n a rTe tis e h t o t e ta g y lb m e s s A e s U e c n a n e tn ia M ria p e R tn e m e c a lp e R tn e m h s ib ru fe R y g re n e la n o ita re p Oe s u re ta w la n o ita re p Oe s u n o itc u rts n o c ­e Dn o itilo m e d tro p s n a rT g n is s e c o rp e ts a W la s o p s iD ­e s u e R­y re v o c e R­g n ilc y c e Rla itn e to p
A1 A2 A3 A4 A5 B1 B2 B3 B4 B5 B6 B7 C1 C2 C3 C4 D
X X X X X MND MND MNR MNR MNR MND MND X X X X X
RESULTS OF THE LCA - ENVIRONMENTAL IMPACT according to EN 15804+A2: 1 m² of installed PU insulation board with 50
µm aluminium facing
Parameter Unit A1-A3 A4 A5 C1 C2 C3 C4 D
GWP­total kg CO 2 eq 1.44E+01 4.57E­01 1.86E­01 0 8.97E­02 8.64E+00 0 ­4.37E+00
GWP­fossil kg CO 2 eq 1.44E+01 4.52E­01 1.83E­01 0 8.86E­02 8.64E+00 0 ­4.36E+00
GWP­biogenic kg CO 2 eq ­5.92E­02 1.06E­03 3.03E­03 0 2.07E­04 1.14E­03 0 ­1.44E­02
GWP­luluc kg CO 2 eq 1.11E­02 4.27E­03 1.95E­07 0 8.38E­04 2.18E­05 0 ­3.69E­04
ODP kg CFC11 eq 1.25E­11 4.04E­14 9.07E­15 0 7.92E­15 2.06E­12 0 ­2.67E­11
AP mol H+ eq 3.4E­02 6.01E­04 2.15E­05 0 1.18E­04 5.2E­03 0 ­8.15E­03
EP­freshwater kg P eq 5.03E­05 1.68E­06 2.19E­09 0 3.3E­07 4.65E­07 0 ­5.77E­06
EP­marine kg N eq 7.97E­03 2.12E­04 5.66E­06 0 4.15E­05 2.48E­03 0 ­1.94E­03
EP­terrestrial mol N eq 8.28E­02 2.54E­03 1.04E­04 0 4.99E­04 2.85E­02 0 ­2.09E­02
kg NMVOC
POCP 4.26E­02 5.19E­04 1.6E­05 0 1.02E­04 6.38E­03 0 ­5.54E­03
eq
ADPE kg Sb eq 1.4E­06 3E­08 8.44E­11 0 5.88E­09 1.81E­08 0 ­2.81E­07
ADPF MJ 3.46E+02 6.27E+00 2.32E­02 0 1.23E+00 3.83E+00 0 ­7.48E+01
m3 world eq
WDP 2.2E+00 5.32E­03 1.68E­02 0 1.04E­03 8.61E­01 0 ­3.73E­01
deprived
GWP = Global warming potential; ODP = Depletion potential of the stratospheric ozone layer; AP = Acidification potential of land and water; EP =
Eutrophication potential; POCP = Formation potential of tropospheric ozone photochemical oxidants; ADPE = Abiotic depletion potential for non­fossil
resources; ADPF = Abiotic depletion potential for fossil resources; WDP = Water (user) deprivation potential)
RESULTS OF THE LCA - INDICATORS TO DESCRIBE RESOURCE USE according to EN 15804+A2: 1 m² of installed PU
insulation board with 50 µm aluminium facing
Parameter Unit A1-A3 A4 A5 C1 C2 C3 C4 D
PERE MJ 2.76E+01 4.44E­01 2.68E+00 0 8.71E­02 1.36E+00 0 ­2.25E+01
PERM MJ 2.68E+00 0 ­2.68E+00 0 0 0 0 0
PERT MJ 3.03E+01 4.44E­01 5.79E­03 0 8.71E­02 1.36E+00 0 ­2.25E+01
PENRE MJ 2.28E+02 6.29E+00 2.14E+01 0 1.23E+00 1.01E+02 0 ­7.49E+01
PENRM MJ 1.18E+02 0 ­2.14E+01 0 0 ­9.71E+01 0 0
PENRT MJ 3.46E+02 6.29E+00 2.32E­02 0 1.23E+00 3.83E+00 0 ­7.49E+01
SM kg 0 0 0 0 0 0 0 0
RSF MJ 0 0 0 0 0 0 0 0
NRSF MJ 0 0 0 0 0 0 0 0
FW m3 1.15E­01 4.89E­04 3.95E­04 0 9.59E­05 2.06E­02 0 ­2.44E­02
PERE = Use of renewable primary energy excluding renewable primary energy resources used as raw materials; PERM = Use of renewable primary
energy resources used as raw materials; PERT = Total use of renewable primary energy resources; PENRE = Use of non­renewable primary energy
excluding non­renewable primary energy resources used as raw materials; PENRM = Use of non­renewable primary energy resources used as raw
materials; PENRT = Total use of non­renewable primary energy resources; SM = Use of secondary material; RSF = Use of renewable secondary fuels;
NRSF = Use of non­renewable secondary fuels; FW = Use of net fresh water
RESULTS OF THE LCA – WASTE CATEGORIES AND OUTPUT FLOWS according to EN 15804+A2:
1 m² of installed PU insulation board with 50 µm aluminium facing
Parameter Unit A1-A3 A4 A5 C1 C2 C3 C4 D
HWD kg 1.04E­07 2.33E­11 6.4E­13 0 4.56E­12 7.71E­11 0 ­3.71E­09
NHWD kg 9.44E­01 9.06E­04 7.91E­04 0 1.78E­04 4.43E­02 0 ­2.9E­01
RWD kg 6.15E­03 8.13E­06 1.36E­06 0 1.59E­06 3.42E­04 0 ­5.78E­03
CRU kg 0 0 0 0 0 0 0 0
MFR kg 0 0 0 0 0 2.67E­01 0 0
MER kg 0 0 0 0 0 0 0 0
EEE MJ 0 0 3.8E­01 0 0 1.48E+01 0 0
6 Environmental Product Declaration ­ IVPU e.V. ­ PU thermal insulation boards with 50 µm aluminium facing
EET MJ 0 0 6.76E­01 0 0 2.65E+01 0 0
HWD = Hazardous waste disposed; NHWD = Non­hazardous waste disposed; RWD = Radioactive waste disposed; CRU = Components for re­use;
MFR = Materials for recycling; MER = Materials for energy recovery; EEE = Exported electrical energy; EET = Exported thermal energy
RESULTS OF THE LCA – additional impact categories according to EN 15804+A2-optional:
1 m² of installed PU insulation board with 50 µm aluminium facing
Parameter Unit A1-A3 A4 A5 C1 C2 C3 C4 D
Disease
PM 3.22E­07 4.99E­09 1.14E­10 0 9.8E­10 1.53E­08 0 ­7.74E­08
incidence
IR kBq U235 eq 8.1E­01 1.17E­03 2.19E­04 0 2.3E­04 5.61E­02 0 ­1.02E+00
ETP­fw CTUe 1.16E+02 4.42E+00 8.94E­03 0 8.66E­01 1.1E+00 0 ­1.23E+01
HTP­c CTUh 4.58E­09 8.9E­11 1.18E­12 0 1.75E­11 8.19E­11 0 ­1.13E­09
HTP­nc CTUh 1.57E­07 3.93E­09 1.03E­11 0 7.71E­10 1.25E­09 0 ­2.58E­08
SQP SQP 4.71E+01 2.62E+00 7.13E­03 0 5.13E­01 1.11E+00 0 ­1.24E+01
PM = Potential incidence of disease due to PM emissions; IR = Potential Human exposure efficiency relative to U235; ETP­fw = Potential comparative
Toxic Unit for ecosystems; HTP­c = Potential comparative Toxic Unit for humans (cancerogenic); HTP­nc = Potential comparative Toxic Unit for humans
(not cancerogenic); SQP = Potential soil quality index
Disclaimer 1 – for the indicator “Potential Human exposure efficiency relative to U235”. This impact category deals mainly with the
eventual impact of low­dose ionizing radiation on human health of the nuclear fuel cycle. It does not consider effects due to possible
nuclear accidents, occupational exposure or radioactive waste disposal in underground facilities. Potential ionizing radiation from the
soil, radon and from some construction materials is also not measured by this indicator.
Disclaimer 2 – for the indicators “abiotic depletion potential for non­fossil resources”, “abiotic depletion potential for fossil resources”,
“water (user) deprivation potential, deprivation­weighted water consumption”, “potential comparative toxic unit for ecosystems”,
“potential comparative toxic unit for humans – cancerogenic”, “Potential comparative toxic unit for humans ­ not cancerogenic”,
“potential soil quality index”. The results of this environmental impact indicator shall be used with care as the uncertainties on these
results are high as there is limited experience with the indicator.
6. LCA: Interpretation
Modules A1­A3: The environmental impacts during the which burn PU cores in order to generate power and steam.
production stage are mainly determined by raw material Additionally, Module D possesses the recycling potential of the
production and processing in Module A1. For nearly all aluminium used.
categories, these impacts can mostly be attributed to the PU
foam (60 % ­ 90 %) and to a lesser extent to the 50 µm The LCA results show high robustness since the primary data,
aluminium facings (10 % ­ 30 %). More specifically, the results they are based on, do not show any outliers in terms of energy
are mainly driven the production of MDI and polyols in almost consumption and product's composition while comparing the
all indicators except for ODP and POCP, where the impacts can contributing companies and sites. All background data are
mainly be attributed to the power mix and the other production sourced from Sphera LCA FE (GaBi ts) databases. With the
expenses, respectively. used data sets a good overall representativity with regards to
completeness, geographical coverage and technological
Module D: The utilization potential for the next product system coverage is ensured.
originates from using primary energy generated from MVAs
7. Requisite evidence
7.2 Isocyanate emission
7.1 VOC emissions In the analysis conducted by the Fraunhofer Institut für
Holzforschung, Wilhelm­Klauditz­Institut WKI (Test report No.
Emission tests on PU boards with 50 µm aluminium facings 861-98), no isocyanate emission could be detected in the 1m³
found that the VOC values are significantly below the limits test chamber. SUPELCO cartridges have been used for
determined by the AgBB scheme (PU Europe Technical detecting MDI. The detection limit is at 10 ng/m³.
Dossier). The tests were conducted by the research 7.3 Formaldehyde
organisations Eurofins (Denmark), VTT (Finland) and Emission tests on PU insulation boards only detected very
Fraunhofer WKI (Germany), Test report No. MAIC­2016­3308, small quantities of formaldehydes (< 3 μg/m³ (PU Europe
among others. Technical Dossier)). This is significantly below the threshold
value of 120 μg/m³ (Class E1).
VOC emissions
Name Value Unit
TVOC (C6 ­ C16) 0 ­ 100 μg/m3
Sum SVOC (C16 ­ C22) 0 ­ 10 μg/m3
R (dimensionless) 0 ­ 0.5 ­
VOC without NIK 0 ­ 100 μg/m3
Carcinogenic Substances ­ μg/m3
8. References
Standards DIN 18234-2
DIN 18234­2:2018­05, Fire safety of large roofs for
7 Environmental Product Declaration ­ IVPU e.V. ­ PU thermal insulation boards with 50 µm aluminium facing
buildings ­ Fire exposure from below ­ Part 2: List of roofs which EN 15804:2012+A2:2019+AC:2021, Sustainability of
fulfil the requirements of DIN 18234­1; roof areas without construction works — Environmental Product Declarations —
openings. Core rules for the product category of construction products.
DIN 4108-4 prEN 16783:2022-12 - draft
DIN 4108­4:2020­11, Thermal insulation and energy economy Thermal insulation products ­ Environmental Product
in buildings ­ Part 4: Hygrothermal design values. Declarations (EPD) ­ Product Category Rules (PCR)
complementary to EN 15804 for factory made and in­situ
DIN 4108-10 formed products
DIN 4108­10:2021­11, Thermal insulation and energy economy
in buildings ­ Part 10: Application­related requirements for ISO 14025
thermal insulation materials ­ Factory­made products. EN ISO 14025:2011, Environmental labels and declarations —
Type III environmental declarations — Principles and
EN 12091 procedures.
EN 12091:2013­06, Thermal insulating products for building
applications ­ Determination of freeze­thaw resistance. Further References
EN 13165 AgBB
EN 13165:2016­09, Thermal insulation products for buildings – Evaluation scheme for VOCs from construction products;
Factory­made rigid polyurethane foam (PU) products ­ approach for assessing health risks caused by volatile organic
Specification; German version EN 13165:2012. (This norm compounds (VOCs and SVOCs) from construction products,
covers polyurethane rigid foam (PUR) and polyisocyanurate version 2021.
rigid foam (PIR)).
Waste Catalogue Ordinance
EN 13501-1 Waste Catalogue Ordinance of 10 December 2001 (Federal
EN 13501­1:2019­05, Fire classification of construction Law Gazette I p. 3379), last amended by Article 2 of the
products and building elements ­ Part 1: Classification using Ordinance of 24 July 2002 (Federal Law Gazette 2833)
data from reaction to fire tests; German version EN 13501­
1:2007+A1:2010. CPR
Regulation (EU) No. 305/2011 of the European Parliament and
EN 14308 of the Council of 9 March 2011
EN 14308:2016­03, Thermal insulation products for building laying down harmonised condition for the marketing of
equipment and industrial installations ­ Factory made rigid construction products and repealing Council Directive
polyurethane foam (PUR) and polyisocyanurate foam (PIR) 89/106/EC.
products.
EXCLI Journal
EN 15801 Hoffmann, Hans­Dieter; Schupp, Thomas: 'Evaluation of
EN 15801:2010­04, Conservation of cultural property ­ Test consumer risk resulting from exposure against MDI from
methods ­ Determination polyurethane foam,' scientific article, published in the EXCLI
of water absorption by capillarity. Journal in 2009.
EN 1606 IBS 316052507-A
DIN EN 1606:2013­05, Thermal insulating products for building IBS Linz: Test report No. 316052507­A, dated 06.04.2017
applications ­ Determination of compressive creep. (IVPU), "Report on the classification of fire resistance of a rafter
roof with PU over­rafter insulation".
EN 1607
EN 1607:2013­05, Thermal insulating products for building IBU 2021
applications ­ Institut Bauen und Umwelt e.V.: General Instructions for
Determination of tensile strength perpendicular to faces. theEPD programme of Institut Bauen und Umwelt e.V.,
Version2.0, Berlin: Institut Bauen und Umwelt e.V., 2021
EN 16516 www.ibu­epd.com
EN 16516:2020­10, Construction products: Assessment of
release of dangerous substances ­ Determination of emissions IVPU news:
into indoor air. Article "Report on emission of volatile components from PUR
rigid foam insulation products," no. 64 dated June 1999.
EN 29052-1 PCR Part A
EN 29052­1:1992­08, Acoustics; determination of dynamic PCR ­ Part A: Calculation rules for the Life Cycle Assessment
stiffness; part 1: materials used under floating floors in and Requirements on the BackgroundReport, version 1.3,
dwellings. Institut Bauen und Umwelt e.V., 2021.
EN 826 PCR Part B
EN 826:2013­05, Thermal insulating products for building PCR ­ Part B: Requirements of the EPD for foam plastics
applications ­ Determination of compression behaviour. insulation materials, v8, 2021 www.bau­umwelt.de
EN 12088 PU Europe Technical Dossier
EN 12088:2013, Thermal insulating products for building Technical Dossier for amendment to mandate M103
applications ­ Determination of long term water absorption by VOC/SVOC emissions, doc. 13/241, 2013.
diffusion.
Ordinance on Biocide Products No. 528/2012
EN 15804 Regulation (EU) No. 528/2012 of the European Parliament and
8 Environmental Product Declaration ­ IVPU e.V. ­ PU thermal insulation boards with 50 µm aluminium facing
of the Council of 22 May 2012 concerning the making available Test report No. 861-98
on the market and use of biocidal products. Fraunhofer Institut für Holzforschung, Wilhelm­Klauditz­Institut
(WKI): Test report No. 861­98, dated 07.12.1998 (IVPU), "Test
REACH Regulation reports on emissions of volatile components from polyurethan
(EC) No. 1907/2006 of the European Parliament and of the insulating materials".
Council dated 18th December 2006 on the Registration,
Evaluation, Authorisation and Restriction of Chemicals Test report No. MAIC-2016-3308
(REACH). Fraunhofer Institut für Holzforschung, Wilhelm­Klauditz­Institut
(WKI): Test report No. MAIC­2016­3308, dated 04.08.2016 (PU
Sphera LCA FE (GaBi ts) Europe), "Evaluation of emissions data from PU insulation on a
Sphera LCA for Experts, LCA FE, software­system and Commission proposal for the classification of emissions from
databases, Managed LCA content MLC (fka GaBi database), building products in the European Union".
University of Stuttgart and Sphera Solutions GmbH, 2023 CUP
Version: 2023.2., MLC data set documentation under TRGS 900
https://sphera.com/product­sustainability­gabi­data­search/ Federal Institute for Occupational Safety and Health: Technical
(March 2024). Rules for Hazardous Substances (TRGS) 900, Threshold
values for workplaces, 2006, last modified 15.01.2024.
9 Environmental Product Declaration ­ IVPU e.V. ­ PU thermal insulation boards with 50 µm aluminium facing
Publisher
Institut Bauen und Umwelt e.V. +49 (0)30 3087748­ 0
Hegelplatz 1 info@ibu­epd.com
10117 Berlin www.ibu­epd.com
Germany
Programme holder
Institut Bauen und Umwelt e.V. +49 (0)30 3087748­ 0
Hegelplatz 1 info@ibu­epd.com
10117 Berlin www.ibu­epd.com
Germany
Author of the Life Cycle Assessment
Sphera Solutions GmbH +49 (0)711 341817­0
Hauptstraße 111­ 113 info@sphera.com
70771 Leinfelden­Echterdingen www.sphera.com
Germany
Owner of the Declaration
IVPU ­ Industrieverband Polyurethan­Hartschaum +49 711 29 17 16
e.V. ivpu@ivpu.de
Heilbronner Str. 154 http://www.ivpu.de/
70191 Stuttgart
Germany
10 Environmental Product Declaration ­ IVPU e.V. ­ PU thermal insulation boards with 50 µm aluminium facing
