ENVIRONMENTAL PRODUCT DECLARATION
as per ISO 14025 and EN 15804+A2
Owner of the Declaration Schüco International KG
Publisher Institut Bauen und Umwelt e.V. (IBU)
Programme holder Institut Bauen und Umwelt e.V. (IBU)
Declaration number EPD-SCH-20230392-CBA1-EN
Issue date 23.10.2023
Valid to 22.10.2028
Schüco Ultra Low Carbon Aluminium Profile
Schüco International KG
www.ibu-epd.com | https://epd-online.com
General Information
Schüco International KG Schüco Ultra Low Carbon Aluminium Profile
Programme holder Owner of the declaration
IBU – Institut Bauen und Umwelt e.V. Schüco International KG
Hegelplatz 1 Karolinenstraße 1-15
10117 Berlin 33609 Bielefeld
Germany Germany
Declaration number Declared product / declared unit
EPD-SCH-20230392-CBA1-EN 1 kg plate finish, Schüco Ultra Low Carbon aluminium profile
This declaration is based on the product category rules: Scope:
Products of aluminium and aluminium alloys, 01.08.2021 The present environmental product declaration concerns the 1 kg plate
(PCR checked and approved by the SVR) finished Schüco Ultra Low Carbon aluminium profile.
This EPD is based on data from aluminium pressing plants which produce
Issue date aluminium profiles with comparable environmental attributes. The creation
of these aluminium profiles requires technically similar production
23.10.2023
processes.
In this EPD, upstream aluminium production refers to a mixture of primary
Valid to
and secondary aluminium, the proportions have been determined using a
22.10.2028 conservative approach.
The data collected for this EPD refers to 2022.
The owner of the declaration shall be liable for the underlying information
and evidence; the IBU shall not be liable with respect to manufacturer
information, life cycle assessment data and evidences.
The EPD was created according to the specifications of EN 15804+A2. In
the following, the standard will be simplified as EN 15804.
Verification
Dipl.-Ing. Hans Peters The standard EN 15804 serves as the core PCR
(Chairman of Institut Bauen und Umwelt e.V.)
Independent verification of the declaration and data according to ISO
14025:2011
internally X externally
Florian Pronold Matthias Schulz,
(Managing Director Institut Bauen und Umwelt e.V.) (Independent verifier)
1 Environmental Product Declaration - Schüco International KG - Schüco Ultra Low Carbon Aluminium Profile
Product
Product description/Product definition Technical Data
The Ultra Low Carbon aluminium profiles are a semi-finished Physical properties of aluminium (e.g. EN AW-6060/6063; EN
product for use in Schüco windows, doors and façade systems. AW-6005):
Constructional data
Ultra Low Carbon Aluminium Profiles are made from aluminium
Name Value Unit
billets that have a specific environmental quality. According to
Schüco's definition, this quality includes aluminium billets that Gross density 2700 kg/m3
do not surpass a defined global warming potential and contains Melting point 660 °C
a minimum post-consumer scrap content of 75%.
Thermal conductivity 200 W/(mK)
Compliance with the required quality (GWP & 75% post-
Modulus of elasticity 70000 N/mm2
consumer scrap) is verified by the billet suppliers in the form of
an EPD. Shear modulus 27000 N/mm2
Specific heat capacity 0.9 kJ/kgK
The Schüco Ultra Low Carbon aluminium profiles are made out Hardness 65 HB
of aluminium alloys consisting of light metal aluminium (Al) and
Yield strength Rp 0,2 min. 160 N/mm2
various alloying elements (such as silicon, copper, manganese,
magnesium etc.). Tensile strength Rm min. 200 N/mm2
Tensile stress at break 8 %
The raw aluminium profiles can be anodised, wet or powder-
Construction data (as in PCR B: Requirements on the EPD for
coated (as required by the customer).
Products of aluminum and aluminum alloys listed, e.g. electrical
conductivity, coefficient of thermal expansion and the chemical
Relevant standards
composition) are not relevant for this product.
Whether aluminium profiles are subject to harmonisation
regulations or not depends on whether these carry a load in the
Profiles and constructions in accordance with CPR (hEN):
final application (e.g. window frames or support beams).
Performance values of the products corresponding to the
However, since the aluminium profiles are intermediate
Declaration of Performance in relation to its essential features
products, it is not possible to make a clear statement about
as per:
their final application. For this reason, both standards ("Profiles
and constructions in accordance with CPR" and "Profiles that • EN 15088, Aluminium and aluminium alloys – Structural
are not subject to the EU harmonisation regulations") are listed products for construction works –Technical conditions
below in order to cover the scope of the possible end uses of for inspection and delivery
the aluminium profiles. • EN 1090-3, Execution of steel structures and aluminium
structures - Part 3: Technical requirements for
Profiles and constructions in accordance with CPR (hEN): The aluminium structures
regulation (EU) No. 305/2011 (CPR) applies to bringing the
product into circulation in the European Union/European Free Profiles that are not subject to any EU harmonisation
Trade Association (EU/EFTA) (with the exception of legislation: Performance values of the product in regard to its
Switzerland). The product requires a Declaration of features in accordance with the controlled technical regulations
Performance taking into account the following standards: (no CE marking).
• EN 15088, Aluminium and aluminium alloys – Structural
Delivery condition
products for construction works –Technical conditions
Materials delivered in accordance with EN 755-1 or
for inspection and delivery
EN 12020-1. The alloys comply with EN 573-3 regarding their
• EN 1090-3, Execution of steel structures and aluminium
chemical composition. The aluminium profiles are packaged in
structures - Part 3: Technical requirements for
accordance with customer requirements.
aluminium structures
Base materials/Ancillary materials
With regard to use, the respective national regulations apply.
The chemical composition of aluminum alloys of the 6000
series - AlMgSi (specifically EN AW-6060/6063; EN AW-6005)
Profiles that are not subject to any EU harmonisation
can be found in standard EN 573-3 (limit values for alloying
legislation:
elements). The aluminum content is > 90%. The other alloy
With regard to using the product, the respective national
components are magnesium, silicon, iron, copper, manganese,
regulations apply for the location of application
chromium, zinc, titanium.
• EN 755-1, Aluminium and aluminium alloys – Extruded
rod/bar, tube and profiles –Part 1: Technical conditions Material note: Aluminium is a light metal. The melting point of
for inspection and delivery pure aluminium is 660 °C. The natural colour is silvery-white.
• EN 12020-1, Aluminium and aluminium alloys -
Extruded precision profiles in alloys EN AW-6060 and Aluminium is very corrosion-resistant and has a long service
EN AW-6063 - Part 1: Technical conditions for life. A naturally thin oxide layer protects the material from
inspection and delivery degradation due to air, water or certain chemicals.
The properties make it possible to manufacture profiles with
Application complex shapes.
Schüco Ultra Low Carbon aluminium profiles are used in
Schüco windows, doors and façade systems. This product/article/at least one partial article contains
substances listed in the candidate list (date: 28.09.2023)
2 Environmental Product Declaration - Schüco International KG - Schüco Ultra Low Carbon Aluminium Profile
exceeding 0.1 percentage by mass: no. risks to water, air/the atmosphere or soil.
This product/article/at least one partial article contains other The specifications regarding use and maintenance do not
CMR substances in categories 1A or 1B which are not on the comply with the semi-finished product created but instead are
candidate list, exceeding 0.1 percentage by mass: no. specific to the design and intended application of the end
product.
Biocide products were added to this construction product or it
has been treated with biocide products (this then concerns a Reference service life
treated product as defined by the (EU) Ordinance on Biocide An expected life cycle is not declared for aluminium profiles as
Products No. 528/2012): no. these are semi-finished products. The service life is dependent
on the product application. As aluminium is protected by an
Manufacture oxide layer on the surface itself, the service life is, in theory,
Cutting – The aluminium billets are cut to size. unlimited.
Heating – The aluminium billets are heated in an oven to Exceptional fire effects
between 460 °C and 530 °C so that it is easier to reach the In accordance with DIN 4102-4, uncoated aluminium profiles
plastic state of the metal during shaping. fulfil the requirements of building material class A, "non-
flammable". The melting point of the aluminium material is 660
Extrusion – With typical compression of 6000–8000 MN/mm² on °C.
a cross-sectional area of the billet, the hot aluminium billet is • Smoke gas development: No smoke gas develops with
pressed through a pre-heated die. This is how the profile gets the profiles.
its geometric shape. • Burning drops of liquid: Not applicable
• Toxicity of combustion gases: Not applicable
Chilling – The profiles are cooled directly after the extrusion
(there are various processes that use air, water or spray). Water
Cooling is necessary for the final adhesive strength. The exposure of the profiles to water does not lead to any
changes in the product nor to any negative consequences for
Elongation – After extrusion the profiles are elongated in order the environment.
to straighten them out. Cutting to length – Cutting the profiles
according to customer requirements (default 6000 mm). Mechanical destruction
Mechanical destruction is not relevant for aluminium profiles.
Tempering – Hardening of the profiles at a temperature
between 145 °C and 210 °C (5–12 hours). Period of post use
Aluminium profiles are fully recyclable. The material does not
Packaging – This is followed by packing the profiles in suffer any loss in quality from this process. Scrap from
accordance with customer requirements. demolitions, conversions or renovations can be easily
separated and (via the recycling industry) fed into the recycling
Environment and health & safety during manufacture process.
Throughout the entire manufacturing process, all legal
obligations regarding occupational health and safety and the All of the process scrap that occurs during the manufacture and
environment are fulfilled. further processing of the profile in the factory is collected and
processed into new primary material (billets, bars, ...) in a
Production fabrication/installation recycling process in the remelting plant. These billets are then
Throughout the entire manufacturing process, all legal used in the plant as a new starting material.
obligations regarding occupational health and safety and the
environment are fulfilled. Disposal
In accordance with the European Waste Catalogue (EWC) the
Packaging end product complies with the disposal code (170402
All profiles are individually packaged in accordance with Aluminium).
customer requirements. The packing materials used range from
reusable containers, untreated wooden crates and pallets to Due to its high value as a raw material, aluminium scrap is not
cardboard packaging etc. disposed of. Instead, it is fed into an established circle of reuse
or recycling.
In order to protect the profiles, they are packaged separately
with cardboard intermediate layers, polyethylene (PE) foil and
paper, for example. The PE foil, paper and cardboard used can
be fed into the recycling process by the customer.
Condition during use
The profiles are made of an alloy which consists of aluminium
and the named alloying components. The constituents
correspond to the raw materials named in EN 573-3 with the
specified mass percentage shares.
There are no special features of the material composition for
the period of use.
Environment and health & safety during use
The intended use of the aluminium profiles does not pose any
3 Environmental Product Declaration - Schüco International KG - Schüco Ultra Low Carbon Aluminium Profile
LCA: Calculation rules
separation of materials.
Declared Unit
The declared unit refers to 1 kg of extruded aluminium profile. Module C2 includes transportation of post-consumer waste to
Declared unit and mass reference waste processing.
Name Value Unit
Module C3 does not include environmental impacts, as
Declared unit 1 kg
aluminium waste reaches its end-of-waste status after
Geographically, the study represents the production of dismantling.
aluminium extrusion profiles in Central Europe. Upstream
aluminium production refers to European production and a Module C4 does not include environmental impacts, as all 100
mixture of primary and secondary aluminium. The proportions % of the waste is expected to be recycled.
of primary and secondary aluminium have been determined
using a conservative approach. Module D includes potential benefits from all net flows given in
modules A5 and C3 that leave the system boundary of the
System boundary product system after having past end-of-waste state in the form
Cradle to gate with options: modules A1–A3, C, D and of recovery and/or recycling potentials.
additional modules A4 and A5
Geographic Representativeness
Modules A1 to A3 include the supply of all materials, auxiliaries, Land or region, in which the declared product system is
energy and packaging materials up to the factory gate, as well manufactured, used or handled at the end of the product´s
as waste processing up to the end-of-waste state or disposal of lifespan: Europe
final residues. Aluminium billets, produced from remelted
production scrap, stay within the product system and are
Comparability
reused within A3.
Basically, a comparison or an evaluation of EPD data is only
possible if all the data sets to be compared were created
Module A4 includes transport of the aluminium profile to the
according to EN 15804 and the building context, respectively
place of installation or further processing.
the product-specific characteristics of performance, are taken
into account. LCAfE software and MLC databases (f.k.a. GaBi)
Module A5 includes the disposal of packaging material.
by Sphera Solutions GmbH were used for all background
databases and LCA calculations.
Module C1 includes the energy demand for dismantling and
LCA: Scenarios and additional technical information
End of Life (C1-C4)
Characteristic product properties of biogenic carbon
For dismantling and separation of built-in aluminium profiles at
The product itself does not contain any biogenic Carbon.
the end of life, the use of diesel-powered construction
Packaging material contain biogenic carbon from the use of
machinery is assumed in module C1.
wood and cardboard/ paper.
Name Value Unit
Note: 1 kg of biogenic carbon is equivalent to 44/12 kg of CO 2. Diesel used in construction machines (C1) 0.0056 kg
Information on biogenic carbon content at factory gate Transport distance in module C2 is considered with the listed
Name ValueUnit scenario settings.
kg Name Value Unit
Biogenic carbon content in product -
C Litres of fuel (C2) 0.0029 l/100km
Biogenic carbon content in accompanying kg Transport distance (C2) 50 km
0.021
packaging C Capacity utilisation (including empty runs) 61 %
The following technical information is a basis for the declared
modules or can be used for developing specific scenarios in the Collection rate of aluminium scrap at the end of life is set to 100
context of a building assessment. %.
Name Value Unit
Transport to the building site (A4) Collected separately waste type (aluminium) 1 kg
Name Value Unit
Reuse, recovery and/or recycling potentials (D), relevant
Litres of fuel (A4) 0.0029 l/100km
scenario information
Transport distance (A4) 100 km
Recycling potentials are calculated for the amount of the net
Capacity utilisation (including empty runs) 61 %
flow aluminium scrap.
Installation into the building (A5) Name Value Unit
Name ValueUnit Net flow aluminium scrap 0.23 kg
Output substances following waste treatment on
0.056 kg
site packaging waste
4 Environmental Product Declaration - Schüco International KG - Schüco Ultra Low Carbon Aluminium Profile
LCA: Results
DESCRIPTION OF THE SYSTEM BOUNDARY (X = INCLUDED IN LCA; MND = MODULE OR INDICATOR NOT DECLARED; MNR
= MODULE NOT RELEVANT)
Benefits and
Construction loads beyond
Product stage Use stage End of life stage
process stage the system
boundaries
la ire ta m w a Ry lp p u s tro p s n a rT g n iru tc a fu n a M e h t m o rf tro p s n a rTe tis e h t o t e ta g y lb m e s s A e s U e c n a n e tn ia M ria p e R tn e m e c a lp e R tn e m h s ib ru fe R y g re n e la n o ita re p Oe s u re ta w la n o ita re p Oe s u n o itc u rts n o c -e Dn o itilo m e d tro p s n a rT g n is s e c o rp e ts a W la s o p s iD -e s u e R-y re v o c e R-g n ilc y c e Rla itn e to p
A1 A2 A3 A4 A5 B1 B2 B3 B4 B5 B6 B7 C1 C2 C3 C4 D
X X X X X MND MND MNR MNR MNR MND MND X X X X X
RESULTS OF THE LCA - ENVIRONMENTAL IMPACT according to EN 15804+A2: 1 kg Schüco Ultra Low Carbon Aluminium
Profile
Parameter Unit A1-A3 A4 A5 C1 C2 C3 C4 D
GWP-total kg CO 2 eq 2.27E+00 8.69E-03 9.78E-02 1.99E-02 4.34E-03 0 0 -1.48E+00
GWP-fossil kg CO 2 eq 2.33E+00 8.58E-03 2.22E-02 1.96E-02 4.29E-03 0 0 -1.47E+00
GWP-biogenic kg CO 2 eq -6.04E-02 2.54E-05 7.57E-02 7.73E-05 1.27E-05 0 0 -4.8E-03
GWP-luluc kg CO 2 eq 8.8E-04 7.96E-05 3.61E-07 1.81E-04 3.98E-05 0 0 -2.88E-04
ODP kg CFC11 eq 1.75E-11 1.12E-15 9.19E-15 2.55E-15 5.59E-16 0 0 -1.22E-11
AP mol H+ eq 8.4E-03 1.28E-05 1.74E-05 1.15E-04 6.4E-06 0 0 -5.73E-03
EP-freshwater kg P eq 2.91E-06 3.14E-08 2.64E-09 7.16E-08 1.57E-08 0 0 -7.75E-07
EP-marine kg N eq 1.62E-03 4.67E-06 5.36E-06 5.6E-05 2.34E-06 0 0 -8.16E-04
EP-terrestrial mol N eq 1.76E-02 5.52E-05 7.6E-05 6.2E-04 2.76E-05 0 0 -8.87E-03
kg NMVOC
POCP 4.78E-03 1.12E-05 1.46E-05 1.49E-04 5.62E-06 0 0 -2.52E-03
eq
ADPE kg Sb eq 9.79E-07 5.66E-10 8.54E-11 1.29E-09 2.83E-10 0 0 -4.06E-07
ADPF MJ 3.47E+01 1.17E-01 2.34E-02 2.67E-01 5.85E-02 0 0 -2.13E+01
m3 world eq
WDP 1.64E-01 1.04E-04 1.07E-02 2.37E-04 5.19E-05 0 0 -6.54E-02
deprived
GWP = Global warming potential; ODP = Depletion potential of the stratospheric ozone layer; AP = Acidification potential of land and water; EP =
Eutrophication potential; POCP = Formation potential of tropospheric ozone photochemical oxidants; ADPE = Abiotic depletion potential for non-fossil
resources; ADPF = Abiotic depletion potential for fossil resources; WDP = Water (user) deprivation potential)
RESULTS OF THE LCA - INDICATORS TO DESCRIBE RESOURCE USE according to EN 15804+A2: 1 kg Schüco Ultra Low
Carbon Aluminium Profile
Parameter Unit A1-A3 A4 A5 C1 C2 C3 C4 D
PERE MJ 1.48E+01 8.52E-03 7.88E-01 1.94E-02 4.26E-03 0 0 -1.03E+01
PERM MJ 7.82E-01 0 -7.82E-01 0 0 0 0 0
PERT MJ 1.55E+01 8.52E-03 5.79E-03 1.94E-02 4.26E-03 0 0 -1.03E+01
PENRE MJ 3.44E+01 1.17E-01 3.27E-01 2.68E-01 5.87E-02 0 0 -2.14E+01
PENRM MJ 3.04E-01 0 -3.04E-01 0 0 0 0 0
PENRT MJ 3.47E+01 1.17E-01 2.34E-02 2.68E-01 5.87E-02 0 0 -2.14E+01
SM kg 9.54E-01 0 0 0 0 0 0 2.31E-01
RSF MJ 0 0 0 0 0 0 0 0
NRSF MJ 0 0 0 0 0 0 0 0
FW m3 2.24E-02 9.33E-06 2.52E-04 2.13E-05 4.66E-06 0 0 -1.77E-02
PERE = Use of renewable primary energy excluding renewable primary energy resources used as raw materials; PERM = Use of renewable primary
energy resources used as raw materials; PERT = Total use of renewable primary energy resources; PENRE = Use of non-renewable primary energy
excluding non-renewable primary energy resources used as raw materials; PENRM = Use of non-renewable primary energy resources used as raw
materials; PENRT = Total use of non-renewable primary energy resources; SM = Use of secondary material; RSF = Use of renewable secondary fuels;
NRSF = Use of non-renewable secondary fuels; FW = Use of net fresh water
RESULTS OF THE LCA – WASTE CATEGORIES AND OUTPUT FLOWS according to EN 15804+A2:
1 kg Schüco Ultra Low Carbon Aluminium Profile
Parameter Unit A1-A3 A4 A5 C1 C2 C3 C4 D
HWD kg 1.86E-08 3.64E-13 5.97E-13 8.29E-13 1.82E-13 0 0 -1.33E-08
NHWD kg 5.3E-01 1.79E-05 1.89E-03 4.08E-05 8.95E-06 0 0 -4.35E-01
RWD kg 3.07E-03 2.2E-07 1.31E-06 5.01E-07 1.1E-07 0 0 -2.42E-03
CRU kg 0 0 0 0 0 0 0 0
MFR kg 0 0 1E-04 0 0 1E+00 0 0
MER kg 0 0 0 0 0 0 0 0
EEE MJ 0 0 1.18E-01 0 0 0 0 0
EET MJ 0 0 2.11E-01 0 0 0 0 0
5 Environmental Product Declaration - Schüco International KG - Schüco Ultra Low Carbon Aluminium Profile
HWD = Hazardous waste disposed; NHWD = Non-hazardous waste disposed; RWD = Radioactive waste disposed; CRU = Components for re-use;
MFR = Materials for recycling; MER = Materials for energy recovery; EEE = Exported electrical energy; EET = Exported thermal energy
RESULTS OF THE LCA – additional impact categories according to EN 15804+A2-optional:
1 kg Schüco Ultra Low Carbon Aluminium Profile
Parameter Unit A1-A3 A4 A5 C1 C2 C3 C4 D
Disease
PM 1.34E-07 1.06E-10 1.07E-10 2.29E-09 5.3E-11 0 0 -9.17E-08
incidence
IR kBq U235 eq 5.97E-01 3.28E-05 2.09E-04 7.47E-05 1.64E-05 0 0 -4.88E-01
ETP-fw CTUe 1.15E+01 8.31E-02 1.1E-02 1.89E-01 4.16E-02 0 0 -8.05E+00
HTP-c CTUh 8.91E-10 1.7E-12 8.97E-13 3.87E-12 8.51E-13 0 0 -3.95E-10
HTP-nc CTUh 4.94E-08 9.07E-11 4.96E-11 2.55E-10 4.54E-11 0 0 -1.05E-08
SQP SQP 1.24E+01 4.89E-02 7.04E-03 1.11E-01 2.45E-02 0 0 -6.91E-01
PM = Potential incidence of disease due to PM emissions; IR = Potential Human exposure efficiency relative to U235; ETP-fw = Potential comparative
Toxic Unit for ecosystems; HTP-c = Potential comparative Toxic Unit for humans (cancerogenic); HTP-nc = Potential comparative Toxic Unit for humans
(not cancerogenic); SQP = Potential soil quality index
Disclaimer 1 – for the indicator “Potential Human exposure efficiency relative to U235”. This impact category deals mainly with the
eventual impact of low-dose ionizing radiation on human health of the nuclear fuel cycle. It does not consider effects due to possible
nuclear accidents, occupational exposure or radioactive waste disposal in underground facilities. Potential ionizing radiation from the
soil, radon and from some construction materials is also not measured by this indicator.
Disclaimer 2 – for the indicators “abiotic depletion potential for non-fossil resources”, “abiotic depletion potential for fossil resources”,
“water (user) deprivation potential, deprivation-weighted water consumption”, “potential comparative toxic unit for ecosystems”,
“potential comparative toxic unit for humans – cancerogenic”, “Potential comparative toxic unit for humans - not cancerogenic”,
“potential soil quality index”. The results of this environmental impact indicator shall be used with care as the uncertainties on these
results are high as there is limited experience with the indicator.
References
Standards of 18 December 2014 amending Decision 2000/532/EC on the
list of waste pursuant to Directive 2008/98/EC of the European
DIN 4102-4 Parliament and of the Council.
DIN 4102-4:2016-05, Fire behaviour of building materials and
building components - Part 4: Synopsis and application of ISO 14025
classified building materials, components and special EN ISO 14025:2011, Environmental labels and declarations —
components. Type III environmental declarations — Principles and
procedures.
EN 573-3
EN 573-3:2019-10, Aluminium and aluminium alloys - Chemical Regulation (EU) No. 305/2011 (CPR)
composition and form of wrought products - Part 3: Chemical REGULATION (EU) No 305/2011 OF THE EUROPEAN
composition and form of products. PARLIAMENT AND OF THE COUNCIL, of 9 March 2011, laying
down harmonised conditions for the marketing of construction
EN 755-1 products and repealing Council Directive 89/106/EEC.
EN 755-1:2016-10, Aluminium and aluminium alloys – Extruded
rod/bar, tube and profiles –Part 1: Technical conditions for Schüco Standard 62
inspection and delivery. Schüco Standard 62, Technical Delivery Conditions for
Extruded Aluminium Profiles.
EN 1090-3
EN1090-3:2019, Execution of steel structures and aluminium Further References
structures - Part 3: Technical requirements for aluminium
structures. EPD: Aluminiumprofil pressblank
Umwelt-Produktdeklaration: Aluminiumprofil pressblank.
EN 12020-1 Aluminium Deutschland, EPD-GDA-20190068-IBH2-DE. Berlin:
EN 12020-1:2022, Aluminium and aluminium alloys - Extruded Institut Bauen und Umwelt e.V. (Hrsg.), 13.11.2019.
precision profiles in alloys EN AW-6060 and EN AW-6063 - Part
1: Technical conditions for inspection and delivery. IBU 2021
Institut Bauen und Umwelt e.V.: General Instructions for the
EN 15088 EPD programme of Institut Bauen und Umwelt e.V., Version
EN 15088:2006-03, Aluminium and aluminium alloys – 2.0, Berlin: Institut Bauen und Umwelt e.V., https://ibu-
Structural products for construction works –Technical conditions epd.com/, 2021.
for inspection and delivery.
IBU PCR Part A
EN 15804 PCR - Part A: Calculation Rules for the Life Cycle Assessment
EN15804:2012+A2:2019+AC:2021, Sustainability of and Requirements on the Project Report according to EN
construction works — Environmental Product Declarations — 15804+A2:2019, version 1.3, Institut Bauen und Umwelt e.V.,
Core rules for the product category of construction products. https://ibu-epd.com/, 2022.
IBU PCR Part B
EWC PCR – Part B: Requirements of the EPD for products of
European Waste Catalogue (EWC), COMMISSION DECISION aluminium and aluminium alloys, version 7, 24/07/2023, Institut
6 Environmental Product Declaration - Schüco International KG - Schüco Ultra Low Carbon Aluminium Profile
Bauen und Umwelt e.V., https://ibu-epd.com/, 2021. CUP 2023.1. Sphera Solutions GmbH,
https://sphera.com/product-sustainability-gabi-data-search/,
LCAfE software and MLC databases 2023.
LCAfE and MLC databases (f.k.a. GaBi) by Sphera. Version
7 Environmental Product Declaration - Schüco International KG - Schüco Ultra Low Carbon Aluminium Profile
Publisher
Institut Bauen und Umwelt e.V. +49 (0)30 3087748- 0
Hegelplatz 1 info@ibu-epd.com
10117 Berlin www.ibu-epd.com
Germany
Programme holder
Institut Bauen und Umwelt e.V. +49 (0)30 3087748- 0
Hegelplatz 1 info@ibu-epd.com
10117 Berlin www.ibu-epd.com
Germany
Author of the Life Cycle Assessment
Sphera Solutions GmbH +49 (0)711 341817-0
Hauptstraße 111- 113 info@sphera.com
70771 Leinfelden-Echterdingen www.sphera.com
Germany
Owner of the Declaration
Schüco International KG +49 (0)521 78 30
Karolinenstraße 1-15 info@schueco.com
33609 Bielefeld www.schueco.com
Germany
8 Environmental Product Declaration - Schüco International KG - Schüco Ultra Low Carbon Aluminium Profile
