ENVIRONMENTAL PRODUCT DECLARATION
as per ISO 14025 and EN 15804+A2
Owner of the Declaration VELUX Group
Publisher Institut Bauen und Umwelt e.V. (IBU)
Programme holder Institut Bauen und Umwelt e.V. (IBU)
Declaration number EPD-VEL-20230512-CBJ2-EN
Issue date 11.03.2024
Valid to 10.03.2029
VELUX roof balcony and terrace window
VELUX Group
www.ibu-epd.com | https://epd-online.com
General Information
VELUX Group VELUX roof balcony and terrace window
Programme holder Owner of the declaration
IBU – Institut Bauen und Umwelt e.V. VELUX Group
Hegelplatz 1 Ådalsvej 99
10117 Berlin 2970 Hørsholm
Germany Denmark
Declaration number Declared product / declared unit
EPD-VEL-20230512-CBJ2-EN The declared unit is a roof balcony and terrace window of 1 m2 with triple
glazing configuration (3-layer). The declared unit is based on the standard
size 1.23 m x 1.48 m (EN 17213:2020).
This declaration is based on the product category rules: Scope:
Windows and doors , 01.08.2021 The EPD is a representative EPD covering VELUX terrace and balcony
(PCR checked and approved by the SVR) windows as specified in more detail in the product description. The
products are manufactured by the VELUX Group at production sites in
different locations in Europe for sale throughout Europe. The windows' final
Issue date assembly take place in Denmark.
The owner of the declaration shall be liable for the underlying information
11.03.2024
and evidence; the IBU shall not be liable with respect to manufacturer
information, life cycle assessment data and evidences.
Valid to
The EPD was created according to the specifications of EN 15804+A2. In
10.03.2029 the following, the standard will be simplified as EN 15804.
Verification
The standard EN 15804 serves as the core PCR
Independent verification of the declaration and data according to ISO
14025:2011
internally X externally
Dipl.-Ing. Hans Peters
(Chairman of Institut Bauen und Umwelt e.V.)
Florian Pronold Dr.-Ing. Nikolay Minkov,
(Managing Director Institut Bauen und Umwelt e.V.) (Independent verifier)
1 Environmental Product Declaration - VELUX Group - VELUX roof balcony and terrace window
Product
The performance values are specific for each standard wooden
Product description/Product definition roof window variant covered by the EPD. The declared values
The VELUX roof balcony and terrace are skylight window in the table relate to the reference product including the
products for sale in the European market. The product family variants GEL and VEA with triple-glazed configuration 65G. The
covers a range of product varieties as specified in the table technical data between the variants GEL and VEA differ only for
below. "impact resistance". For other covered product variants, specific
The terrace window consists of a combination between the GEL values can be selected at the bottom of the above-mentioned
variant (top) and either VEA, VEB or VEC variants (bottom). download page.
The terrace window is available in one size (2.45 m x 0.78 m),
Constructional data
while the different variants in the window are not available as
individual windows. The balcony window (GDL) consists of an Name Value Unit
upper and a lower section. All windows have a wooden Reaction to fire (both
C-s1,d2 class
frame/sash. Some windows can be opened (venting), while variants)
others cannot be opened (fixed). In addition, the windows Air permeability acc. EN
3 class
consist of 4 different hinge-functionalities (pivot-hung, top-hung, 12207 (both variants)
side-hung, bottom-hung). The handles and handlebars are
Resistance to wind load, (for
made of aluminium, while the hinges are made of steel
window width >1140 mm or
(galvanised, stainless). The windows are opened and closed
height > 1398 mm no C3 class
manually. The calculations are based on the representative
performance is determined)
terrace window type named GEL+VEA. In the LCA, the GEL
(both variants)
+VEA was assessed to be a conservative choice for a
4 (toughened) - 11 - 3
representative window type.
Resistance to snow loads (heat strengthened) -
mm
(both variants) 11 - 6.8 (laminated
The glass panes are with triple glazing (3-layer glazing unit)
float)
and different glass configurations are covered by the EPD. The
glass thickness ranges from 10 to 13 mm. The glass panes Water tightness acc. EN
have cavities filled with Krypton gas. The EPD is based on a 12208 unprotected / protected 9A class
weighted average of the included glazing unit configurations. (both variants)
The included glazing unit configurations are: 65 G and 66. Impact resistance (for window
width <550 mm or height
3 class
Only the window modules are included, which means that any <778 mm no performance is
applied installation products, accessories, etc. are not part of determined) (variant GEL)
the EPD. These are available as separate EPDs, that can be Impact resistance (for window
used in combination with this EPD. width <550 mm or height
NPD class
<778 mm no performance is
determined) (variant VEA)
Acoustic performance (both
35 (-1; -4) -
variants)
Load-bearing capacity of
passed -
safety devices (both variants)
Thermal transmittance, 90
degree installation acc. to EN 1.0 W/(m2K)
10077-1/2 (both variants)
Solar factor (both variants) 0.44 -
Light transmittance (both
0.62 -
1 3-layer glazing options: 65 G, 66 variants)
Product performance data in accordance with DS/EN 14351-
For the placing on the market of the product in the European
1:2006+A2:2016, Windows and doors - Product standard,
Union/European Free Trade Association (EU/EFTA) (with the
performance characteristics - Part 1: Windows and external
exception of Switzerland) Regulation (EU) No. 305/2011 (CPR)
pedestrian doorsets.
applies. The product needs a declaration of performance taking
into consideration EN 14351-1:2006+A2:2016, Windows and Base materials/Ancillary materials
doors - Product standard, performance characteristics - Part 1: The main components of the roof balcony and terrace are the
Windows and external pedestrian doorsets. For the application glazing unit (made of mainly laminated and tempered glass),
and use, the respective national provisions apply. wooden frames/sashes (made of wood), hinges (made of steel)
and handles/handlebars (made of aluminium). The packaging
Application
of the products consists of mostly cardboard and wood along
VELUX roof balcony and terrace are used in renovation and
with paper inserts, EPS (expanded polystyrene), PE LD and
new build. Either installed as a single window or in a galvanised steel. The total weight of 1 m2 roof balcony and
combination of multiple windows.
terrace (including the sales packaging) is 56.45 kg.
Technical Data
The Declaration of Performance including relevant technical
specifications and test methods/test standards can be
downloaded from the website: www.velux.com/ce
2 Environmental Product Declaration - VELUX Group - VELUX roof balcony and terrace window
Name Value Unit cladding, drilling etc.). For the glazing units, VELUX receives
the glazing unit components from suppliers and produces the
Glazing unit (3-layer) 43 %
final glazing units at a site located in Denmark. After their
Wooden frame/sash 23 %
production, the glazing units join the window assembly process.
Steel components (galvanised and stainless) 12 %
Finally, the frames/sashes, glazing unit, and the rest of the
Other components (including packaging) 23 % components (delivered by suppliers) are transported to VELUX
Recycled content of aluminium 30 % assembly site in Denmark, where they are assembled into the
Recycled content of steel 10 % final window product.
Recycled content of glass 12 %
This product/article/at least one partial article contains
The wooden components (sashes, frames) are produced substances listed in the candidate list (date: 23.08.2023)
internally in VELUX facilities, located in Hungary, Poland, and exceeding 0.1 percentage by mass: NO.
Denmark. VELUX receives sawn pine wood (dried) and
processes it (sawing, cutting etc.) into lamellas of different Reference service life
quality. The lamellas are then glued together (lamination) and No reference service life (RSL) is defined for the roof windows
processed into profiles (cutting them into the correct size, because the use stage modules are not included in the EPD.
LCA: Calculation rules
• A3 - Manufacturing: The wooden frames/sashes and
Declared Unit glazing units are produced internally at VELUX
Multiple product dimensions are represented by this EPD as production sites. Subsequently, the final production and
specified in the product description. The declared unit is 1 m2 assembly of the windows takes place, which involves
roof balcony and terrace calculated based on the standard activities such as shortening of profiles, drilling of holes,
window size (1.23 m x 1.48 m based on EN 17213.2020) with clamping and glueing, mounting of gaskets, brackets,
triple glazed window panes (65 G, 66). Since the frame/sash panes etc.
construction is alike across all variants in the product group, the
parts that set the variants apart are primarily the window- End of life stage:
operation components, such as hinges, handles and ventilation
• C1 - De-construction/demolition: deconstruction of the
flaps. These components are to a high degree metal-based,
window with the use of an electric screwdriver and
and the worst-case product can thus be identified by the weight
manual work.
of products with similar size and glazing unit. The heavier the
• C2 - Transport: transport of window materials to Material
product, the larger the content of metal. The variant GEL
Recovery Facilities (MRF) and then to incineration,
combined with VEA (GEL+VEA) present the largest weight per
landfill or recycling facilities.
m2 across the product group of terrace windows and the
• C3 - Waste processing: sorting of waste, recycling
balcony window GDL. Therefore, the GEL combined with VEA
(metal and glass waste), incineration (plastic and wood
variant can be considered more representative as worst-case
waste) and landfill (metal, glass, wood and plastic
scenario for the whole windows product group.
waste).
Declared unit and mass reference • C4 - Disposal: disposal of all materials
Name Value Unit
Benefits and loads beyond the system boundaries:
Declared unit 1 m2
• D - Reuse, recovery and recycling potential: benefits
Grammage 49.58 kg/m2
from plastic and wood waste incineration processes and
Layer thickness (glazing unit) 0.0393 m material recycling of metal and glass.
Data quality and sensitivity analysis show that the results are
robust with regard to data quality and appropriateness. There is For the environmental impact, the use of green electricity was
low variability of production processes and product variations calculated taking into account the residual electricity mix for the
have a limited influence on the results. remaining electricity. The proportion of the electricity demand
covered by green electricity in the total electricity demand is
System boundary 79.23 %.
The type of the EPD is "cradle to gate - with options" including
Geographic Representativeness
the modules C1-C4 and D. The following life cycle phases were
considered: Land or region, in which the declared product system is
manufactured, used or handled at the end of the product´s
Product stage: lifespan: Europe
• A1 - Raw material supply: extraction and processing,
production of the pre-products (e.g. laminated glass, Comparability
sawn pine wood, metal/plastic components, sealants Basically, a comparison or an evaluation of EPD data is only
etc.) and sales packaging components (e.g., possible if all the data sets to be compared were created
cardboard). according to EN 15804 and the building context, respectively
• A2 - Transport: Transport of pre-products and packaging the product-specific characteristics of performance, are taken
components to the processing or assembly sites, as well into account. Average secondary datasets were retrieved from
as internal transportation of components between sites. the Managed LCA Content (v2021.2) and Ecoinvent (v3.8)
databases.
LCA: Scenarios and additional technical information
Characteristic product properties of biogenic carbon
3 Environmental Product Declaration - VELUX Group - VELUX roof balcony and terrace window
12.82 kg of wood is used in window frames/sashes and 0.07 kg
End of life (C1-C4)
of paper inlet is used per declared unit. For the packaging, 3.51
Name ValueUnit
kg of cardboard, 3.26 kg of wood and 0.03 kg of paper insert
are used per declared unit. Collected as mixed construction waste 49.52 kg
Recycling 16.76 kg
Information on describing the biogenic carbon content at
factory gate Energy recovery 15.58 kg
Name ValueUnit Landfilling 17.18 kg
kg Omitted to atmosphere (Krypton gas in glazing unit) 0.065 kg
Biogenic carbon content in product 5.88
C
Reuse, recovery and/or recycling potentials (D), relevant
Biogenic carbon content in accompanying kg
4.11 scenario information
packaging C
Name Value Unit
Wood incinerated 95 %
Note: 1 kg of biogenic carbon is equivalent to 44/12 kg of CO .
2 Plastic incinerated 95 %
Paper incinerated 95 %
Note: 1 kg of biogenic carbon is equivalent to 44/12 kg of CO .
2
Metal recycled 95 %
Glass recycled 30 %
The construction process stage and the use stage modules are
not declared. However, the quantity of packaging generated in
module A5 is declared as scenario information.
Scenario information for packaging generated in module
A5
Name Value Unit
Cardboard packaging for waste treatment 3.51 kg
EPS packaging for waste treatment 0.04 kg
Steel packaging for waste treatment (galvanised) 0.02 kg
Paper packaging for waste treatment 0.03 kg
PE LD packaging for waste treatment 0.004 kg
Wood packaging for waste treatment 3.26 kg
4 Environmental Product Declaration - VELUX Group - VELUX roof balcony and terrace window
LCA: Results
DESCRIPTION OF THE SYSTEM BOUNDARY (X = INCLUDED IN LCA; MND = MODULE OR INDICATOR NOT DECLARED; MNR
= MODULE NOT RELEVANT)
Benefits and
Construction loads beyond
Product stage Use stage End of life stage
process stage the system
boundaries
la ire ta m w a Ry lp p u s tro p s n a rT g n iru tc a fu n a M e h t m o rf tro p s n a rTe tis e h t o t e ta g y lb m e s s A e s U e c n a n e tn ia M ria p e R tn e m e c a lp e R tn e m h s ib ru fe R y g re n e la n o ita re p Oe s u re ta w la n o ita re p Oe s u n o itc u rts n o c -e Dn o itilo m e d tro p s n a rT g n is s e c o rp e ts a W la s o p s iD -e s u e R-y re v o c e R-g n ilc y c e Rla itn e to p
A1 A2 A3 A4 A5 B1 B2 B3 B4 B5 B6 B7 C1 C2 C3 C4 D
X X X MND MND MND MND MNR MNR MNR MND MND X X X X X
RESULTS OF THE LCA - ENVIRONMENTAL IMPACT according to EN 15804+A2: 1 m2 VELUX standard wooden roof window
Parameter Unit A1 A2 A3 C1 C2 C3 C4 D
GWP-total kg CO 2 eq 9.64E+01 4.76E-01 5.33E+01 1.97E-03 2.92E+00 2.73E+01 4.05E+00 -4.49E+01
GWP-fossil kg CO 2 eq 1.41E+02 4.73E-01 4.04E+01 1.97E-03 2.87E+00 6.94E+00 3.01E-01 -4.48E+01
GWP-biogenic kg CO 2 eq -4.52E+01 -5.59E-04 1.28E+01 1.1E-06 3.09E-02 2.03E+01 3.75E+00 -8.15E-02
GWP-luluc kg CO 2 eq 1.03E-01 3.85E-03 4.69E-02 3.38E-07 2.37E-02 1.46E-03 7.59E-04 -1.55E-02
ODP kg CFC11 eq 1.25E-06 9.31E-17 1.13E-07 2.22E-17 5.73E-16 -6.47E-09 1.08E-15 -9.69E-14
AP mol H+ eq 5.84E-01 5.43E-04 9.86E-02 3.18E-06 1.75E-02 7.06E-03 2.04E-03 -1.65E-01
EP-freshwater kg P eq 5.49E-03 1.4E-06 5.98E-04 7.92E-10 8.62E-06 -1.41E-05 4.31E-06 -2.53E-05
EP-marine kg N eq 1.18E-01 1.76E-04 3.5E-02 8.43E-07 8.54E-03 2.88E-03 5.75E-04 -3.16E-02
EP-terrestrial mol N eq 1.31E+00 2.07E-03 3.56E-01 9.03E-06 9.45E-02 3.64E-02 6.09E-03 -3.48E-01
kg NMVOC
POCP 3.33E-01 4.78E-04 8.98E-02 2.39E-06 1.58E-02 7.78E-03 2.07E-03 -8.81E-02
eq
ADPE kg Sb eq 2.01E-03 4.18E-08 4.27E-05 2.44E-10 2.57E-07 5.82E-08 2.67E-08 -1.11E-05
ADPF MJ 1.96E+03 6.29E+00 6.16E+02 4.08E-02 3.87E+01 1.04E+01 4.03E+00 -5.62E+02
m3 world eq
WDP 1.17E+01 4.37E-03 2.13E+00 1.58E-04 2.69E-02 3E+00 3.1E-02 -3.4E+00
deprived
GWP = Global warming potential; ODP = Depletion potential of the stratospheric ozone layer; AP = Acidification potential of land and water; EP =
Eutrophication potential; POCP = Formation potential of tropospheric ozone photochemical oxidants; ADPE = Abiotic depletion potential for non-fossil
resources; ADPF = Abiotic depletion potential for fossil resources; WDP = Water (user) deprivation potential)
RESULTS OF THE LCA - INDICATORS TO DESCRIBE RESOURCE USE according to EN 15804+A2: 1 m2 VELUX standard
wooden roof window
Parameter Unit A1 A2 A3 C1 C2 C3 C4 D
PERE MJ 3.9E+02 3.61E-01 1.18E+03 4.21E-03 2.22E+00 1.98E+02 4.92E-01 -1.31E+02
PERM MJ 4.45E+02 0 1.21E+02 0 0 -1.96E+02 0 0
PERT MJ 8.35E+02 3.61E-01 1.3E+03 4.21E-03 2.22E+00 1.83E+00 4.92E-01 -1.31E+02
PENRE MJ 1.82E+03 6.31E+00 6.15E+02 4.09E-02 3.88E+01 1.09E+02 4.04E+00 -5.64E+02
PENRM MJ 1.36E+02 0 1.55E+00 0 0 -9.86E+01 0 0
PENRT MJ 1.96E+03 6.31E+00 6.17E+02 4.09E-02 3.88E+01 1.04E+01 4.04E+00 -5.64E+02
SM kg 4.62E+00 0 0 0 0 0 0 0
RSF MJ 0 0 0 0 0 0 0 0
NRSF MJ 0 0 0 0 0 0 0 0
FW m3 7.97E-01 4.13E-04 1.35E-01 9.2E-06 2.55E-03 7.09E-02 9.34E-04 -3.04E-01
PERE = Use of renewable primary energy excluding renewable primary energy resources used as raw materials; PERM = Use of renewable primary
energy resources used as raw materials; PERT = Total use of renewable primary energy resources; PENRE = Use of non-renewable primary energy
excluding non-renewable primary energy resources used as raw materials; PENRM = Use of non-renewable primary energy resources used as raw
materials; PENRT = Total use of non-renewable primary energy resources; SM = Use of secondary material; RSF = Use of renewable secondary fuels;
NRSF = Use of non-renewable secondary fuels; FW = Use of net fresh water
RESULTS OF THE LCA – WASTE CATEGORIES AND OUTPUT FLOWS according to EN 15804+A2:
1 m2 VELUX standard wooden roof window
Parameter Unit A1 A2 A3 C1 C2 C3 C4 D
HWD kg 2.92E-03 3.32E-10 3.88E-05 4.91E-12 2.04E-09 1.73E-09 4.89E-10 -5.98E-08
NHWD kg 1.22E+01 9.89E-04 6.79E-01 7.68E-06 6.09E-03 1.56E+00 1.66E+01 -5.51E+00
RWD kg 5.67E-02 1.14E-05 3.01E-02 6.61E-06 7.04E-05 4.22E-04 4.32E-05 -2.6E-02
CRU kg 0 0 0 0 0 0 0 0
MFR kg 1.67E-02 0 2.17E+01 0 0 1.68E+01 0 0
MER kg 0 0 0 0 0 1.53E+01 0 0
EEE MJ 3.33E-02 0 0 0 0 4.51E+01 0 0
EET MJ 4.85E-02 0 0 0 0 8.21E+01 0 0
5 Environmental Product Declaration - VELUX Group - VELUX roof balcony and terrace window
HWD = Hazardous waste disposed; NHWD = Non-hazardous waste disposed; RWD = Radioactive waste disposed; CRU = Components for re-use;
MFR = Materials for recycling; MER = Materials for energy recovery; EEE = Exported electrical energy; EET = Exported thermal energy
RESULTS OF THE LCA – additional impact categories according to EN 15804+A2-optional:
1 m2 VELUX standard wooden roof window
Parameter Unit A1 A2 A3 C1 C2 C3 C4 D
Disease
PM 1.16E-05 4.35E-09 9.71E-07 2.9E-11 7.56E-08 6.15E-08 2.44E-08 -1.65E-06
incidence
IR kBq U235 eq 1.16E+01 1.67E-03 3.03E+00 9.66E-04 1.03E-02 5.43E-02 4.9E-03 -4.92E+00
ETP-fw CTUe 2E+03 4.67E+00 1.68E+02 1.25E-02 2.87E+01 5.81E+00 2.85E+00 -2.21E+02
HTP-c CTUh 1E-06 9.44E-11 2.84E-08 2.09E-13 5.8E-10 2.64E-10 3.05E-10 -3.21E-08
HTP-nc CTUh 2.23E-06 4.9E-09 5.44E-07 1.16E-11 3.56E-08 1.72E-08 3.43E-08 -3.84E-07
SQP SQP 8.24E+03 2.16E+00 1.38E+03 3.39E-03 1.33E+01 1.78E+00 7.05E-01 -3.23E+01
PM = Potential incidence of disease due to PM emissions; IR = Potential Human exposure efficiency relative to U235; ETP-fw = Potential comparative
Toxic Unit for ecosystems; HTP-c = Potential comparative Toxic Unit for humans (cancerogenic); HTP-nc = Potential comparative Toxic Unit for humans
(not cancerogenic); SQP = Potential soil quality index
Disclaimer 1 – for the indicator 'Potential Human exposure efficiency relative to U235'. This impact category deals mainly with the
eventual impact of low-dose ionizing radiation on human health of the nuclear fuel cycle. It does not consider effects due to possible
nuclear accidents, occupational exposure or radioactive waste disposal in underground facilities. Potential ionizing radiation from the
soil, radon and from some construction materials is also not measured by this indicator.
Disclaimer 2 – for the indicators 'abiotic depletion potential for non-fossil resources', 'abiotic depletion potential for fossil resources',
'water (user) deprivation potential, deprivation-weighted water consumption', 'potential comparative toxic unit for ecosystems', 'potential
comparative toxic unit for humans – cancerogenic', 'Potential comparative toxic unit for humans - not cancerogenic', 'potential soil
quality index'. The results of this environmental impact indicator shall be used with care as the uncertainties on these results are high
as there is limited experience with the indicator.
The results show that module A1 has the highest impact across all environmental impact indicators (except GWP – biogenic). Module
A3 has the second highest impact in most impact indicators due to the energy consumption and the use of residual electricity grid mix.
All main components in the windows contribute significantly to some of the environmental indicators, except for wood, which is only
significant for the GWP-luluc and WDP indicators. The glass in the glazing units has the highest contribution in most impact categories
among all material types. The galvanized steel components contribute significantly to the results due to their high weight contribution to
the product. The aluminium components are also significant for the WDP indicator, although the weight of the aluminium components is
notably lower in comparison with the galvanized steel components. This is most likely due to the relatively high energy and water
consumption in the production of aluminium. It is noted that the production activities at VELUX contribute significantly to the GWP-fossil
and ADPF impact indicators therefore, the actual impact contribution of the final wooden components is higher than the impact of
upstream processed wood production.
References
IBU PCR Part A
IBU PCR Part A: Institut Bauen und Umwelt e.V., Product ISO 14025
Category Rules for Building-Related Products and Services. DIN EN ISO 14025:2011-10, Environmental labels and
Calculation Rules for the Life Cycle Assessment and declarations - Type III environmental declarations - Principles
Requirements on the Project Report according to EN and procedures.
15804+A2:2019, version 1.3.
EN 14351-1
IBU PCR Part B EN 14351-1:2006+A2:2016, Windows and doors - Product
IBU PCR Part B: Institut Bauen und Umwelt e.V., Requirements standard, performance characteristics - Part 1: Windows and
on the EPD for Windows and doors, version 1.4: 2021. external pedestrian doorsets.
IBU 2021 EN 15804
IBU 2021 Institut Bauen und Umwelt e.V.: General Instructions EN 15804:2012+A2:2019+AC:2021, Sustainability of
for the EPD programme of Institut Bauen und Umwelt e.V. construction works — Environmental Product Declarations —
Version 2.0, Berlin: Institut Bauen und Umwelt e.V., 2021. Core rules for the product category of construction products.
www.ibu-epd.com
EN 17213
EN 12207 EN 17213:2020, Windows and doors – Environmental Product
EN 12207:2016 Windows and doors - Air permeability - Declarations – Product category rules for windows and
Classification pedestrian doorsets.
EN 12208 ISO 10077-1
EN 12208:2000 Windows and doors. Watertightness. ISO 10077-1:2017, Thermal performance of windows, doors
Classification is classified in these ICS categories: 91.060.50 and shutters - Calculation of thermal transmittance - Part 1:
Doors and windows General.
EN 13501-1 ISO 10077-2
EN 13501-1 EN13501-1, 2018: Fire classification of ISO 10077-2:2017, Thermal performance of windows, doors
construction products and building elements - Part 1: and shutters - Calculation of thermal transmittance - Part 2:
Classification using data from reaction to fire tests. Numerical method for frames.
6 Environmental Product Declaration - VELUX Group - VELUX roof balcony and terrace window
23.08.2023
Regulation (EU) No 305/2011
Regulation (EU) No 305/2011 of the European Parliament and LCA for Experts (GaBi) LCA software, Managed LCA
of the Council of 9 March 2011 laying down harmonised Content and Ecoinvent databases
conditions for the marketing of construction products The LCA modelling software is LCA for Experts program
andrepealing Council Directive 89/106/EEC version 10.7.1 with corresponding databases from Sphera
Solutions GmbH (Managed LCA Content) and Ecoinvent.
Candidate list Documentation hyperlink www.gabisoftware. com/support/gabi.
ECHA Candidate list of substances of very high concern, status
7 Environmental Product Declaration - VELUX Group - VELUX roof balcony and terrace window
Publisher
Institut Bauen und Umwelt e.V. +49 (0)30 3087748- 0
Hegelplatz 1 info@ibu-epd.com
10117 Berlin www.ibu-epd.com
Germany
Programme holder
Institut Bauen und Umwelt e.V. +49 (0)30 3087748- 0
Hegelplatz 1 info@ibu-epd.com
10117 Berlin www.ibu-epd.com
Germany
Author of the Life Cycle Assessment
FORCE Technology +4543250856
Park Alle 345 chme@forcetechnology.com
2605 Brøndby www.forcetechnology.com
Denmark
Owner of the Declaration
VELUX Group +4545164871
Ådalsvej 99 birthe.kjeldsen@velux.com
2970 Hørsholm www.velux.com
Denmark
8 Environmental Product Declaration - VELUX Group - VELUX roof balcony and terrace window
